@prefix C1901A00006: <http://example.org/au/leg/dataset/C1901A00006/> .
@prefix dcat: <http://www.w3.org/ns/dcat#> .
@prefix dt: <http://purl.org/dc/terms/> .
@prefix legcons: <http://example.org/au/leg/concepts/> .
@prefix owl: <http://www.w3.org/2002/07/owl#> .
@prefix rdfs: <http://www.w3.org/2000/01/rdf-schema#> .
@prefix schema: <https://schema.org/> .
@prefix skos: <http://www.w3.org/2004/02/skos/core#> .
@prefix xsd: <http://www.w3.org/2001/XMLSchema#> .

C1901A00006: a owl:Ontology,
        dcat:Dataset ;
    dt:Agent "Home Affairs"@en-AU ;
    dt:created "2024-08-05T21:40:36.246152"^^xsd:dateTime ;
    dt:creator "https://orcid.org/0009-0007-8434-7325"^^xsd:anyURI ;
    dt:date "2024-07-01T00:00:00+10:00"^^xsd:dateTime ;
    dt:description "Customs Act 1901"@en-AU ;
    dt:identifier "https://www.legislation.gov.au/C1901A00006/latest"^^xsd:anyURI ;
    dt:publisher "Department of Industry, Science and Resources" ;
    dt:source "scheme=AGLSTERMS.AglsAgent; corporateName=Office Parliamentary Counsel; address=Locked Bag 30 Kingston ACT 2604; contact=+61 2 6120 1400"@en-AU ;
    dt:subject "Customs Act 1901"@en-AU ;
    dt:title "Customs Act 1901"@en-AU ;
    owl:imports legcons: ;
    schema:identifier "C1901A00006" ;
    schema:status "In force" ;
    schema:version "C2024C00311 (C182)" .

C1901A00006:10 a legcons:Item,
        skos:Concept,
        dcat:Resource ;
    rdfs:label "Item I10"@en-AU ;
    rdfs:comment "4 B  What is a Customs related law - GraphNodeID: I10"@en-AU ;
    skos:definition "4 B  What is a Customs related law"@en-AU ;
    skos:narrower C1901A00006:2 ;
    skos:prefLabel "Item I10"@en-AU ;
    dcat:accessURL "https://www.legislation.gov.au/C1901A00006/2024-07-01/2024-07-01/text/original/epub/OEBPS/document_1/document_1.html#_Toc172622984"^^xsd:anyURI .

C1901A00006:100 a legcons:Item,
        skos:Concept,
        dcat:Resource ;
    rdfs:label "Item I100"@en-AU ;
    rdfs:comment "67 EA  Special reporters - GraphNodeID: I100"@en-AU ;
    skos:definition "67 EA  Special reporters"@en-AU ;
    skos:narrower C1901A00006:99 ;
    skos:prefLabel "Item I100"@en-AU ;
    dcat:accessURL "https://www.legislation.gov.au/C1901A00006/2024-07-01/2024-07-01/text/original/epub/OEBPS/document_1/document_1.html#_Toc172623074"^^xsd:anyURI .

C1901A00006:1000 a legcons:Item,
        skos:Concept,
        dcat:Resource ;
    rdfs:label "Item I1000"@en-AU ;
    rdfs:comment "203 DA  When seizure warrants for goods in transit can be issued - GraphNodeID: I1000"@en-AU ;
    skos:definition "203 DA  When seizure warrants for goods in transit can be issued"@en-AU ;
    skos:narrower C1901A00006:999 ;
    skos:prefLabel "Item I1000"@en-AU ;
    dcat:accessURL "https://www.legislation.gov.au/C1901A00006/2024-07-01/2024-07-01/text/original/epub/OEBPS/document_3/document_3.html#_Toc172627034"^^xsd:anyURI .

C1901A00006:1001 a legcons:Item,
        skos:Concept,
        dcat:Resource ;
    rdfs:label "Item I1001"@en-AU ;
    rdfs:comment "203 DB  The things that are authorised by seizure warrants for goods in transit - GraphNodeID: I1001"@en-AU ;
    skos:definition "203 DB  The things that are authorised by seizure warrants for goods in transit"@en-AU ;
    skos:narrower C1901A00006:999 ;
    skos:prefLabel "Item I1001"@en-AU ;
    dcat:accessURL "https://www.legislation.gov.au/C1901A00006/2024-07-01/2024-07-01/text/original/epub/OEBPS/document_3/document_3.html#_Toc172627035"^^xsd:anyURI .

C1901A00006:1003 a legcons:Item,
        skos:Concept,
        dcat:Resource ;
    rdfs:label "Item I1003"@en-AU ;
    rdfs:comment "203 E  Conduct of ordinary searches and frisk searches - GraphNodeID: I1003"@en-AU ;
    skos:definition "203 E  Conduct of ordinary searches and frisk searches"@en-AU ;
    skos:narrower C1901A00006:1002 ;
    skos:prefLabel "Item I1003"@en-AU ;
    dcat:accessURL "https://www.legislation.gov.au/C1901A00006/2024-07-01/2024-07-01/text/original/epub/OEBPS/document_3/document_3.html#_Toc172627037"^^xsd:anyURI .

C1901A00006:1004 a legcons:Item,
        skos:Concept,
        dcat:Resource ;
    rdfs:label "Item I1004"@en-AU ;
    rdfs:comment "203 F  Announcement before entry - GraphNodeID: I1004"@en-AU ;
    skos:definition "203 F  Announcement before entry"@en-AU ;
    skos:narrower C1901A00006:1002 ;
    skos:prefLabel "Item I1004"@en-AU ;
    dcat:accessURL "https://www.legislation.gov.au/C1901A00006/2024-07-01/2024-07-01/text/original/epub/OEBPS/document_3/document_3.html#_Toc172627038"^^xsd:anyURI .

C1901A00006:1005 a legcons:Item,
        skos:Concept,
        dcat:Resource ;
    rdfs:label "Item I1005"@en-AU ;
    rdfs:comment "203 G  Details of warrant to be given to occupier - GraphNodeID: I1005"@en-AU ;
    skos:definition "203 G  Details of warrant to be given to occupier"@en-AU ;
    skos:narrower C1901A00006:1002 ;
    skos:prefLabel "Item I1005"@en-AU ;
    dcat:accessURL "https://www.legislation.gov.au/C1901A00006/2024-07-01/2024-07-01/text/original/epub/OEBPS/document_3/document_3.html#_Toc172627039"^^xsd:anyURI .

C1901A00006:1006 a legcons:Item,
        skos:Concept,
        dcat:Resource ;
    rdfs:label "Item I1006"@en-AU ;
    rdfs:comment "203 H  Occupier entitled to be present during search or seizure - GraphNodeID: I1006"@en-AU ;
    skos:definition "203 H  Occupier entitled to be present during search or seizure"@en-AU ;
    skos:narrower C1901A00006:1002 ;
    skos:prefLabel "Item I1006"@en-AU ;
    dcat:accessURL "https://www.legislation.gov.au/C1901A00006/2024-07-01/2024-07-01/text/original/epub/OEBPS/document_3/document_3.html#_Toc172627040"^^xsd:anyURI .

C1901A00006:1007 a legcons:Item,
        skos:Concept,
        dcat:Resource ;
    rdfs:label "Item I1007"@en-AU ;
    rdfs:comment "203 HA  Requirement to provide name or address etc - GraphNodeID: I1007"@en-AU ;
    skos:definition "203 HA  Requirement to provide name or address etc"@en-AU ;
    skos:narrower C1901A00006:1002 ;
    skos:prefLabel "Item I1007"@en-AU ;
    dcat:accessURL "https://www.legislation.gov.au/C1901A00006/2024-07-01/2024-07-01/text/original/epub/OEBPS/document_3/document_3.html#_Toc172627041"^^xsd:anyURI .

C1901A00006:1008 a legcons:Item,
        skos:Concept,
        dcat:Resource ;
    rdfs:label "Item I1008"@en-AU ;
    rdfs:comment "203 J  Availability of assistance and use of force in executing a warrant - GraphNodeID: I1008"@en-AU ;
    skos:definition "203 J  Availability of assistance and use of force in executing a warrant"@en-AU ;
    skos:narrower C1901A00006:1002 ;
    skos:prefLabel "Item I1008"@en-AU ;
    dcat:accessURL "https://www.legislation.gov.au/C1901A00006/2024-07-01/2024-07-01/text/original/epub/OEBPS/document_3/document_3.html#_Toc172627042"^^xsd:anyURI .

C1901A00006:1009 a legcons:Item,
        skos:Concept,
        dcat:Resource ;
    rdfs:label "Item I1009"@en-AU ;
    rdfs:comment "203 K  Specific powers available to executing officers - GraphNodeID: I1009"@en-AU ;
    skos:definition "203 K  Specific powers available to executing officers"@en-AU ;
    skos:narrower C1901A00006:1002 ;
    skos:prefLabel "Item I1009"@en-AU ;
    dcat:accessURL "https://www.legislation.gov.au/C1901A00006/2024-07-01/2024-07-01/text/original/epub/OEBPS/document_3/document_3.html#_Toc172627043"^^xsd:anyURI .

C1901A00006:101 a legcons:Item,
        skos:Concept,
        dcat:Resource ;
    rdfs:label "Item I101"@en-AU ;
    rdfs:comment "67 EB  Requirements for registration as a special reporter - GraphNodeID: I101"@en-AU ;
    skos:definition "67 EB  Requirements for registration as a special reporter"@en-AU ;
    skos:narrower C1901A00006:99 ;
    skos:prefLabel "Item I101"@en-AU ;
    dcat:accessURL "https://www.legislation.gov.au/C1901A00006/2024-07-01/2024-07-01/text/original/epub/OEBPS/document_1/document_1.html#_Toc172623075"^^xsd:anyURI .

C1901A00006:1010 a legcons:Item,
        skos:Concept,
        dcat:Resource ;
    rdfs:label "Item I1010"@en-AU ;
    rdfs:comment "203 L  Use of animals in executing a warrant - GraphNodeID: I1010"@en-AU ;
    skos:definition "203 L  Use of animals in executing a warrant"@en-AU ;
    skos:narrower C1901A00006:1002 ;
    skos:prefLabel "Item I1010"@en-AU ;
    dcat:accessURL "https://www.legislation.gov.au/C1901A00006/2024-07-01/2024-07-01/text/original/epub/OEBPS/document_3/document_3.html#_Toc172627044"^^xsd:anyURI .

C1901A00006:1011 a legcons:Item,
        skos:Concept,
        dcat:Resource ;
    rdfs:label "Item I1011"@en-AU ;
    rdfs:comment "203 M  Warrants by telephone or other electronic means - GraphNodeID: I1011"@en-AU ;
    skos:definition "203 M  Warrants by telephone or other electronic means"@en-AU ;
    skos:narrower C1901A00006:1002 ;
    skos:prefLabel "Item I1011"@en-AU ;
    dcat:accessURL "https://www.legislation.gov.au/C1901A00006/2024-07-01/2024-07-01/text/original/epub/OEBPS/document_3/document_3.html#_Toc172627045"^^xsd:anyURI .

C1901A00006:1012 a legcons:Item,
        skos:Concept,
        dcat:Resource ;
    rdfs:label "Item I1012"@en-AU ;
    rdfs:comment "203 N  Receipts for things seized under warrant - GraphNodeID: I1012"@en-AU ;
    skos:definition "203 N  Receipts for things seized under warrant"@en-AU ;
    skos:narrower C1901A00006:1002 ;
    skos:prefLabel "Item I1012"@en-AU ;
    dcat:accessURL "https://www.legislation.gov.au/C1901A00006/2024-07-01/2024-07-01/text/original/epub/OEBPS/document_3/document_3.html#_Toc172627046"^^xsd:anyURI .

C1901A00006:1013 a legcons:Item,
        skos:Concept,
        dcat:Resource ;
    rdfs:label "Item I1013"@en-AU ;
    rdfs:comment "203 P  Offence for making false statements in warrants - GraphNodeID: I1013"@en-AU ;
    skos:definition "203 P  Offence for making false statements in warrants"@en-AU ;
    skos:narrower C1901A00006:1002 ;
    skos:prefLabel "Item I1013"@en-AU ;
    dcat:accessURL "https://www.legislation.gov.au/C1901A00006/2024-07-01/2024-07-01/text/original/epub/OEBPS/document_3/document_3.html#_Toc172627047"^^xsd:anyURI .

C1901A00006:1014 a legcons:Item,
        skos:Concept,
        dcat:Resource ;
    rdfs:label "Item I1014"@en-AU ;
    rdfs:comment "203 Q  Offences relating to telephone warrants - GraphNodeID: I1014"@en-AU ;
    skos:definition "203 Q  Offences relating to telephone warrants"@en-AU ;
    skos:narrower C1901A00006:1002 ;
    skos:prefLabel "Item I1014"@en-AU ;
    dcat:accessURL "https://www.legislation.gov.au/C1901A00006/2024-07-01/2024-07-01/text/original/epub/OEBPS/document_3/document_3.html#_Toc172627048"^^xsd:anyURI .

C1901A00006:1016 a legcons:Item,
        skos:Concept,
        dcat:Resource ;
    rdfs:label "Item I1016"@en-AU ;
    rdfs:comment "203 R  Retention of things seized as evidential material - GraphNodeID: I1016"@en-AU ;
    skos:definition "203 R  Retention of things seized as evidential material"@en-AU ;
    skos:narrower C1901A00006:1015 ;
    skos:prefLabel "Item I1016"@en-AU ;
    dcat:accessURL "https://www.legislation.gov.au/C1901A00006/2024-07-01/2024-07-01/text/original/epub/OEBPS/document_3/document_3.html#_Toc172627050"^^xsd:anyURI .

C1901A00006:1017 a legcons:Item,
        skos:Concept,
        dcat:Resource ;
    rdfs:label "Item I1017"@en-AU ;
    rdfs:comment "203 S  Magistrate may permit a thing seized as evidential material to be retained - GraphNodeID: I1017"@en-AU ;
    skos:definition "203 S  Magistrate may permit a thing seized as evidential material to be retained"@en-AU ;
    skos:narrower C1901A00006:1015 ;
    skos:prefLabel "Item I1017"@en-AU ;
    dcat:accessURL "https://www.legislation.gov.au/C1901A00006/2024-07-01/2024-07-01/text/original/epub/OEBPS/document_3/document_3.html#_Toc172627051"^^xsd:anyURI .

C1901A00006:1019 a legcons:Item,
        skos:Concept,
        dcat:Resource ;
    rdfs:label "Item I1019"@en-AU ;
    rdfs:comment "203 SA  Subdivision does not apply to seized transit goods - GraphNodeID: I1019"@en-AU ;
    skos:definition "203 SA  Subdivision does not apply to seized transit goods"@en-AU ;
    skos:narrower C1901A00006:1018 ;
    skos:prefLabel "Item I1019"@en-AU ;
    dcat:accessURL "https://www.legislation.gov.au/C1901A00006/2024-07-01/2024-07-01/text/original/epub/OEBPS/document_3/document_3.html#_Toc172627053"^^xsd:anyURI .

C1901A00006:102 a legcons:Item,
        skos:Concept,
        dcat:Resource ;
    rdfs:label "Item I102"@en-AU ;
    rdfs:comment "67 EC  The making of an application - GraphNodeID: I102"@en-AU ;
    skos:definition "67 EC  The making of an application"@en-AU ;
    skos:narrower C1901A00006:99 ;
    skos:prefLabel "Item I102"@en-AU ;
    dcat:accessURL "https://www.legislation.gov.au/C1901A00006/2024-07-01/2024-07-01/text/original/epub/OEBPS/document_1/document_1.html#_Toc172623076"^^xsd:anyURI .

C1901A00006:1020 a legcons:Item,
        skos:Concept,
        dcat:Resource ;
    rdfs:label "Item I1020"@en-AU ;
    rdfs:comment "203 T  Seizure of protected objects - GraphNodeID: I1020"@en-AU ;
    skos:definition "203 T  Seizure of protected objects"@en-AU ;
    skos:narrower C1901A00006:1018 ;
    skos:prefLabel "Item I1020"@en-AU ;
    dcat:accessURL "https://www.legislation.gov.au/C1901A00006/2024-07-01/2024-07-01/text/original/epub/OEBPS/document_3/document_3.html#_Toc172627054"^^xsd:anyURI .

C1901A00006:1021 a legcons:Item,
        skos:Concept,
        dcat:Resource ;
    rdfs:label "Item I1021"@en-AU ;
    rdfs:comment "204  Seized goods to be secured - GraphNodeID: I1021"@en-AU ;
    skos:definition "204  Seized goods to be secured"@en-AU ;
    skos:narrower C1901A00006:1018 ;
    skos:prefLabel "Item I1021"@en-AU ;
    dcat:accessURL "https://www.legislation.gov.au/C1901A00006/2024-07-01/2024-07-01/text/original/epub/OEBPS/document_3/document_3.html#_Toc172627055"^^xsd:anyURI .

C1901A00006:1022 a legcons:Item,
        skos:Concept,
        dcat:Resource ;
    rdfs:label "Item I1022"@en-AU ;
    rdfs:comment "205  Requirement to serve seizure notices - GraphNodeID: I1022"@en-AU ;
    skos:definition "205  Requirement to serve seizure notices"@en-AU ;
    skos:narrower C1901A00006:1018 ;
    skos:prefLabel "Item I1022"@en-AU ;
    dcat:accessURL "https://www.legislation.gov.au/C1901A00006/2024-07-01/2024-07-01/text/original/epub/OEBPS/document_3/document_3.html#_Toc172627056"^^xsd:anyURI .

C1901A00006:1023 a legcons:Item,
        skos:Concept,
        dcat:Resource ;
    rdfs:label "Item I1023"@en-AU ;
    rdfs:comment "205 A  Matters to be dealt with in seizure notices - GraphNodeID: I1023"@en-AU ;
    skos:definition "205 A  Matters to be dealt with in seizure notices"@en-AU ;
    skos:narrower C1901A00006:1018 ;
    skos:prefLabel "Item I1023"@en-AU ;
    dcat:accessURL "https://www.legislation.gov.au/C1901A00006/2024-07-01/2024-07-01/text/original/epub/OEBPS/document_3/document_3.html#_Toc172627057"^^xsd:anyURI .

C1901A00006:1024 a legcons:Item,
        skos:Concept,
        dcat:Resource ;
    rdfs:label "Item I1024"@en-AU ;
    rdfs:comment "205 B  Claim for return of goods seized - GraphNodeID: I1024"@en-AU ;
    skos:definition "205 B  Claim for return of goods seized"@en-AU ;
    skos:narrower C1901A00006:1018 ;
    skos:prefLabel "Item I1024"@en-AU ;
    dcat:accessURL "https://www.legislation.gov.au/C1901A00006/2024-07-01/2024-07-01/text/original/epub/OEBPS/document_3/document_3.html#_Toc172627058"^^xsd:anyURI .

C1901A00006:1025 a legcons:Item,
        skos:Concept,
        dcat:Resource ;
    rdfs:label "Item I1025"@en-AU ;
    rdfs:comment "205 C  Treatment of goods seized if no claim for return is made - GraphNodeID: I1025"@en-AU ;
    skos:definition "205 C  Treatment of goods seized if no claim for return is made"@en-AU ;
    skos:narrower C1901A00006:1018 ;
    skos:prefLabel "Item I1025"@en-AU ;
    dcat:accessURL "https://www.legislation.gov.au/C1901A00006/2024-07-01/2024-07-01/text/original/epub/OEBPS/document_3/document_3.html#_Toc172627059"^^xsd:anyURI .

C1901A00006:1026 a legcons:Item,
        skos:Concept,
        dcat:Resource ;
    rdfs:label "Item I1026"@en-AU ;
    rdfs:comment "205 D  Treatment of goods seized if a claim for return is madegeneral - GraphNodeID: I1026"@en-AU ;
    skos:definition "205 D  Treatment of goods seized if a claim for return is madegeneral"@en-AU ;
    skos:narrower C1901A00006:1018 ;
    skos:prefLabel "Item I1026"@en-AU ;
    dcat:accessURL "https://www.legislation.gov.au/C1901A00006/2024-07-01/2024-07-01/text/original/epub/OEBPS/document_3/document_3.html#_Toc172627060"^^xsd:anyURI .

C1901A00006:1027 a legcons:Item,
        skos:Concept,
        dcat:Resource ;
    rdfs:label "Item I1027"@en-AU ;
    rdfs:comment "205 E  Magistrate may permit goods seized to be retained - GraphNodeID: I1027"@en-AU ;
    skos:definition "205 E  Magistrate may permit goods seized to be retained"@en-AU ;
    skos:narrower C1901A00006:1018 ;
    skos:prefLabel "Item I1027"@en-AU ;
    dcat:accessURL "https://www.legislation.gov.au/C1901A00006/2024-07-01/2024-07-01/text/original/epub/OEBPS/document_3/document_3.html#_Toc172627061"^^xsd:anyURI .

C1901A00006:1028 a legcons:Item,
        skos:Concept,
        dcat:Resource ;
    rdfs:label "Item I1028"@en-AU ;
    rdfs:comment "205 EA  Treatment of goods seized if a claim for return is madesuspected prohibited psychoactive substances - GraphNodeID: I1028"@en-AU ;
    skos:definition "205 EA  Treatment of goods seized if a claim for return is madesuspected prohibited psychoactive substances"@en-AU ;
    skos:narrower C1901A00006:1018 ;
    skos:prefLabel "Item I1028"@en-AU ;
    dcat:accessURL "https://www.legislation.gov.au/C1901A00006/2024-07-01/2024-07-01/text/original/epub/OEBPS/document_3/document_3.html#_Toc172627062"^^xsd:anyURI .

C1901A00006:1029 a legcons:Item,
        skos:Concept,
        dcat:Resource ;
    rdfs:label "Item I1029"@en-AU ;
    rdfs:comment "205 EB  Extending the period for instituting proceedings for recovery of suspected prohibited psychoactive substances - GraphNodeID: I1029"@en-AU ;
    skos:definition "205 EB  Extending the period for instituting proceedings for recovery of suspected prohibited psychoactive substances"@en-AU ;
    skos:narrower C1901A00006:1018 ;
    skos:prefLabel "Item I1029"@en-AU ;
    dcat:accessURL "https://www.legislation.gov.au/C1901A00006/2024-07-01/2024-07-01/text/original/epub/OEBPS/document_3/document_3.html#_Toc172627063"^^xsd:anyURI .

C1901A00006:103 a legcons:Item,
        skos:Concept,
        dcat:Resource ;
    rdfs:label "Item I103"@en-AU ;
    rdfs:comment "67 ED  Consideration of the application - GraphNodeID: I103"@en-AU ;
    skos:definition "67 ED  Consideration of the application"@en-AU ;
    skos:narrower C1901A00006:99 ;
    skos:prefLabel "Item I103"@en-AU ;
    dcat:accessURL "https://www.legislation.gov.au/C1901A00006/2024-07-01/2024-07-01/text/original/epub/OEBPS/document_1/document_1.html#_Toc172623077"^^xsd:anyURI .

C1901A00006:1030 a legcons:Item,
        skos:Concept,
        dcat:Resource ;
    rdfs:label "Item I1030"@en-AU ;
    rdfs:comment "205 EC  Proceedings for recovery of suspected prohibited psychoactive substances - GraphNodeID: I1030"@en-AU ;
    skos:definition "205 EC  Proceedings for recovery of suspected prohibited psychoactive substances"@en-AU ;
    skos:narrower C1901A00006:1018 ;
    skos:prefLabel "Item I1030"@en-AU ;
    dcat:accessURL "https://www.legislation.gov.au/C1901A00006/2024-07-01/2024-07-01/text/original/epub/OEBPS/document_3/document_3.html#_Toc172627064"^^xsd:anyURI .

C1901A00006:1031 a legcons:Item,
        skos:Concept,
        dcat:Resource ;
    rdfs:label "Item I1031"@en-AU ;
    rdfs:comment "205 F  Right of compensation in certain circumstances for goods disposed of or destroyed - GraphNodeID: I1031"@en-AU ;
    skos:definition "205 F  Right of compensation in certain circumstances for goods disposed of or destroyed"@en-AU ;
    skos:narrower C1901A00006:1018 ;
    skos:prefLabel "Item I1031"@en-AU ;
    dcat:accessURL "https://www.legislation.gov.au/C1901A00006/2024-07-01/2024-07-01/text/original/epub/OEBPS/document_3/document_3.html#_Toc172627065"^^xsd:anyURI .

C1901A00006:1032 a legcons:Item,
        skos:Concept,
        dcat:Resource ;
    rdfs:label "Item I1032"@en-AU ;
    rdfs:comment "205 G  Effect of forfeiture - GraphNodeID: I1032"@en-AU ;
    skos:definition "205 G  Effect of forfeiture"@en-AU ;
    skos:narrower C1901A00006:1018 ;
    skos:prefLabel "Item I1032"@en-AU ;
    dcat:accessURL "https://www.legislation.gov.au/C1901A00006/2024-07-01/2024-07-01/text/original/epub/OEBPS/document_3/document_3.html#_Toc172627066"^^xsd:anyURI .

C1901A00006:1033 a legcons:Item,
        skos:Concept,
        dcat:Resource ;
    rdfs:label "Item I1033"@en-AU ;
    rdfs:comment "206  Immediate disposal of certain goods - GraphNodeID: I1033"@en-AU ;
    skos:definition "206  Immediate disposal of certain goods"@en-AU ;
    skos:narrower C1901A00006:1018 ;
    skos:prefLabel "Item I1033"@en-AU ;
    dcat:accessURL "https://www.legislation.gov.au/C1901A00006/2024-07-01/2024-07-01/text/original/epub/OEBPS/document_3/document_3.html#_Toc172627067"^^xsd:anyURI .

C1901A00006:1034 a legcons:Item,
        skos:Concept,
        dcat:Resource ;
    rdfs:label "Item I1034"@en-AU ;
    rdfs:comment "207  Immediate disposal of narcotic goods - GraphNodeID: I1034"@en-AU ;
    skos:definition "207  Immediate disposal of narcotic goods"@en-AU ;
    skos:narrower C1901A00006:1018 ;
    skos:prefLabel "Item I1034"@en-AU ;
    dcat:accessURL "https://www.legislation.gov.au/C1901A00006/2024-07-01/2024-07-01/text/original/epub/OEBPS/document_3/document_3.html#_Toc172627068"^^xsd:anyURI .

C1901A00006:1035 a legcons:Item,
        skos:Concept,
        dcat:Resource ;
    rdfs:label "Item I1035"@en-AU ;
    rdfs:comment "208  Release of goods on security - GraphNodeID: I1035"@en-AU ;
    skos:definition "208  Release of goods on security"@en-AU ;
    skos:narrower C1901A00006:1018 ;
    skos:prefLabel "Item I1035"@en-AU ;
    dcat:accessURL "https://www.legislation.gov.au/C1901A00006/2024-07-01/2024-07-01/text/original/epub/OEBPS/document_3/document_3.html#_Toc172627069"^^xsd:anyURI .

C1901A00006:1036 a legcons:Item,
        skos:Concept,
        dcat:Resource ;
    rdfs:label "Item I1036"@en-AU ;
    rdfs:comment "208 C  Service by post - GraphNodeID: I1036"@en-AU ;
    skos:definition "208 C  Service by post"@en-AU ;
    skos:narrower C1901A00006:1018 ;
    skos:prefLabel "Item I1036"@en-AU ;
    dcat:accessURL "https://www.legislation.gov.au/C1901A00006/2024-07-01/2024-07-01/text/original/epub/OEBPS/document_3/document_3.html#_Toc172627070"^^xsd:anyURI .

C1901A00006:1037 a legcons:Item,
        skos:Concept,
        dcat:Resource ;
    rdfs:label "Item I1037"@en-AU ;
    rdfs:comment "208 D  Disposal of forfeited goods - GraphNodeID: I1037"@en-AU ;
    skos:definition "208 D  Disposal of forfeited goods"@en-AU ;
    skos:narrower C1901A00006:1018 ;
    skos:prefLabel "Item I1037"@en-AU ;
    dcat:accessURL "https://www.legislation.gov.au/C1901A00006/2024-07-01/2024-07-01/text/original/epub/OEBPS/document_3/document_3.html#_Toc172627071"^^xsd:anyURI .

C1901A00006:1038 a legcons:Item,
        skos:Concept,
        dcat:Resource ;
    rdfs:label "Item I1038"@en-AU ;
    rdfs:comment "208 DA  Disposal of narcotic related goods other than narcotic goods - GraphNodeID: I1038"@en-AU ;
    skos:definition "208 DA  Disposal of narcotic related goods other than narcotic goods"@en-AU ;
    skos:narrower C1901A00006:1018 ;
    skos:prefLabel "Item I1038"@en-AU ;
    dcat:accessURL "https://www.legislation.gov.au/C1901A00006/2024-07-01/2024-07-01/text/original/epub/OEBPS/document_3/document_3.html#_Toc172627072"^^xsd:anyURI .

C1901A00006:1039 a legcons:Item,
        skos:Concept,
        dcat:Resource ;
    rdfs:label "Item I1039"@en-AU ;
    rdfs:comment "208 E  Sales subject to conditions - GraphNodeID: I1039"@en-AU ;
    skos:definition "208 E  Sales subject to conditions"@en-AU ;
    skos:narrower C1901A00006:1018 ;
    skos:prefLabel "Item I1039"@en-AU ;
    dcat:accessURL "https://www.legislation.gov.au/C1901A00006/2024-07-01/2024-07-01/text/original/epub/OEBPS/document_3/document_3.html#_Toc172627073"^^xsd:anyURI .

C1901A00006:104 a legcons:Item,
        skos:Concept,
        dcat:Resource ;
    rdfs:label "Item I104"@en-AU ;
    rdfs:comment "67 EE  Basic conditions attaching to registration as a special reporter - GraphNodeID: I104"@en-AU ;
    skos:definition "67 EE  Basic conditions attaching to registration as a special reporter"@en-AU ;
    skos:narrower C1901A00006:99 ;
    skos:prefLabel "Item I104"@en-AU ;
    dcat:accessURL "https://www.legislation.gov.au/C1901A00006/2024-07-01/2024-07-01/text/original/epub/OEBPS/document_1/document_1.html#_Toc172623078"^^xsd:anyURI .

C1901A00006:1040 a legcons:Item,
        skos:Concept,
        dcat:Resource ;
    rdfs:label "Item I1040"@en-AU ;
    rdfs:comment "209  Power to impound certain forfeited goods and release them on payment of duty and penalty - GraphNodeID: I1040"@en-AU ;
    skos:definition "209  Power to impound certain forfeited goods and release them on payment of duty and penalty"@en-AU ;
    skos:narrower C1901A00006:1018 ;
    skos:prefLabel "Item I1040"@en-AU ;
    dcat:accessURL "https://www.legislation.gov.au/C1901A00006/2024-07-01/2024-07-01/text/original/epub/OEBPS/document_3/document_3.html#_Toc172627074"^^xsd:anyURI .

C1901A00006:1041 a legcons:Item,
        skos:Concept,
        dcat:Resource ;
    rdfs:label "Item I1041"@en-AU ;
    rdfs:comment "209 A  Destruction or concealment of evidential material or forfeited goods - GraphNodeID: I1041"@en-AU ;
    skos:definition "209 A  Destruction or concealment of evidential material or forfeited goods"@en-AU ;
    skos:narrower C1901A00006:1018 ;
    skos:prefLabel "Item I1041"@en-AU ;
    dcat:accessURL "https://www.legislation.gov.au/C1901A00006/2024-07-01/2024-07-01/text/original/epub/OEBPS/document_3/document_3.html#_Toc172627075"^^xsd:anyURI .

C1901A00006:1043 a legcons:Item,
        skos:Concept,
        dcat:Resource ;
    rdfs:label "Item I1043"@en-AU ;
    rdfs:comment "209 B  Subdivision applies to seized transit goods - GraphNodeID: I1043"@en-AU ;
    skos:definition "209 B  Subdivision applies to seized transit goods"@en-AU ;
    skos:narrower C1901A00006:1042 ;
    skos:prefLabel "Item I1043"@en-AU ;
    dcat:accessURL "https://www.legislation.gov.au/C1901A00006/2024-07-01/2024-07-01/text/original/epub/OEBPS/document_3/document_3.html#_Toc172627077"^^xsd:anyURI .

C1901A00006:1044 a legcons:Item,
        skos:Concept,
        dcat:Resource ;
    rdfs:label "Item I1044"@en-AU ;
    rdfs:comment "209 C  Seized goods to be secured - GraphNodeID: I1044"@en-AU ;
    skos:definition "209 C  Seized goods to be secured"@en-AU ;
    skos:narrower C1901A00006:1042 ;
    skos:prefLabel "Item I1044"@en-AU ;
    dcat:accessURL "https://www.legislation.gov.au/C1901A00006/2024-07-01/2024-07-01/text/original/epub/OEBPS/document_3/document_3.html#_Toc172627078"^^xsd:anyURI .

C1901A00006:1045 a legcons:Item,
        skos:Concept,
        dcat:Resource ;
    rdfs:label "Item I1045"@en-AU ;
    rdfs:comment "209 D  Requirement to serve seizure notices - GraphNodeID: I1045"@en-AU ;
    skos:definition "209 D  Requirement to serve seizure notices"@en-AU ;
    skos:narrower C1901A00006:1042 ;
    skos:prefLabel "Item I1045"@en-AU ;
    dcat:accessURL "https://www.legislation.gov.au/C1901A00006/2024-07-01/2024-07-01/text/original/epub/OEBPS/document_3/document_3.html#_Toc172627079"^^xsd:anyURI .

C1901A00006:1046 a legcons:Item,
        skos:Concept,
        dcat:Resource ;
    rdfs:label "Item I1046"@en-AU ;
    rdfs:comment "209 E  Matters to be dealt with in seizure notices - GraphNodeID: I1046"@en-AU ;
    skos:definition "209 E  Matters to be dealt with in seizure notices"@en-AU ;
    skos:narrower C1901A00006:1042 ;
    skos:prefLabel "Item I1046"@en-AU ;
    dcat:accessURL "https://www.legislation.gov.au/C1901A00006/2024-07-01/2024-07-01/text/original/epub/OEBPS/document_3/document_3.html#_Toc172627080"^^xsd:anyURI .

C1901A00006:1047 a legcons:Item,
        skos:Concept,
        dcat:Resource ;
    rdfs:label "Item I1047"@en-AU ;
    rdfs:comment "209 F  Application for return of seized goods - GraphNodeID: I1047"@en-AU ;
    skos:definition "209 F  Application for return of seized goods"@en-AU ;
    skos:narrower C1901A00006:1042 ;
    skos:prefLabel "Item I1047"@en-AU ;
    dcat:accessURL "https://www.legislation.gov.au/C1901A00006/2024-07-01/2024-07-01/text/original/epub/OEBPS/document_3/document_3.html#_Toc172627081"^^xsd:anyURI .

C1901A00006:1048 a legcons:Item,
        skos:Concept,
        dcat:Resource ;
    rdfs:label "Item I1048"@en-AU ;
    rdfs:comment "209 G  Status of goods seized if no application for return is made - GraphNodeID: I1048"@en-AU ;
    skos:definition "209 G  Status of goods seized if no application for return is made"@en-AU ;
    skos:narrower C1901A00006:1042 ;
    skos:prefLabel "Item I1048"@en-AU ;
    dcat:accessURL "https://www.legislation.gov.au/C1901A00006/2024-07-01/2024-07-01/text/original/epub/OEBPS/document_3/document_3.html#_Toc172627082"^^xsd:anyURI .

C1901A00006:1049 a legcons:Item,
        skos:Concept,
        dcat:Resource ;
    rdfs:label "Item I1049"@en-AU ;
    rdfs:comment "209 H  Right of compensation for certain goods disposed of or destroyed - GraphNodeID: I1049"@en-AU ;
    skos:definition "209 H  Right of compensation for certain goods disposed of or destroyed"@en-AU ;
    skos:narrower C1901A00006:1042 ;
    skos:prefLabel "Item I1049"@en-AU ;
    dcat:accessURL "https://www.legislation.gov.au/C1901A00006/2024-07-01/2024-07-01/text/original/epub/OEBPS/document_3/document_3.html#_Toc172627083"^^xsd:anyURI .

C1901A00006:105 a legcons:Item,
        skos:Concept,
        dcat:Resource ;
    rdfs:label "Item I105"@en-AU ;
    rdfs:comment "67 EF  Storage and record maintenance conditions - GraphNodeID: I105"@en-AU ;
    skos:definition "67 EF  Storage and record maintenance conditions"@en-AU ;
    skos:narrower C1901A00006:99 ;
    skos:prefLabel "Item I105"@en-AU ;
    dcat:accessURL "https://www.legislation.gov.au/C1901A00006/2024-07-01/2024-07-01/text/original/epub/OEBPS/document_1/document_1.html#_Toc172623079"^^xsd:anyURI .

C1901A00006:1050 a legcons:Item,
        skos:Concept,
        dcat:Resource ;
    rdfs:label "Item I1050"@en-AU ;
    rdfs:comment "209 I  Effect of forfeiture - GraphNodeID: I1050"@en-AU ;
    skos:definition "209 I  Effect of forfeiture"@en-AU ;
    skos:narrower C1901A00006:1042 ;
    skos:prefLabel "Item I1050"@en-AU ;
    dcat:accessURL "https://www.legislation.gov.au/C1901A00006/2024-07-01/2024-07-01/text/original/epub/OEBPS/document_3/document_3.html#_Toc172627084"^^xsd:anyURI .

C1901A00006:1051 a legcons:Item,
        skos:Concept,
        dcat:Resource ;
    rdfs:label "Item I1051"@en-AU ;
    rdfs:comment "209 J  Immediate disposal of unsafe goods - GraphNodeID: I1051"@en-AU ;
    skos:definition "209 J  Immediate disposal of unsafe goods"@en-AU ;
    skos:narrower C1901A00006:1042 ;
    skos:prefLabel "Item I1051"@en-AU ;
    dcat:accessURL "https://www.legislation.gov.au/C1901A00006/2024-07-01/2024-07-01/text/original/epub/OEBPS/document_3/document_3.html#_Toc172627085"^^xsd:anyURI .

C1901A00006:1052 a legcons:Item,
        skos:Concept,
        dcat:Resource ;
    rdfs:label "Item I1052"@en-AU ;
    rdfs:comment "209 K  Disposal of forfeited goods - GraphNodeID: I1052"@en-AU ;
    skos:definition "209 K  Disposal of forfeited goods"@en-AU ;
    skos:narrower C1901A00006:1042 ;
    skos:prefLabel "Item I1052"@en-AU ;
    dcat:accessURL "https://www.legislation.gov.au/C1901A00006/2024-07-01/2024-07-01/text/original/epub/OEBPS/document_3/document_3.html#_Toc172627086"^^xsd:anyURI .

C1901A00006:1053 a legcons:Item,
        skos:Concept,
        dcat:Resource ;
    rdfs:label "Item I1053"@en-AU ;
    rdfs:comment "209 L  Service by post - GraphNodeID: I1053"@en-AU ;
    skos:definition "209 L  Service by post"@en-AU ;
    skos:narrower C1901A00006:1042 ;
    skos:prefLabel "Item I1053"@en-AU ;
    dcat:accessURL "https://www.legislation.gov.au/C1901A00006/2024-07-01/2024-07-01/text/original/epub/OEBPS/document_3/document_3.html#_Toc172627087"^^xsd:anyURI .

C1901A00006:1055 a legcons:Item,
        skos:Concept,
        dcat:Resource ;
    rdfs:label "Item I1055"@en-AU ;
    rdfs:comment "209 M  Application of Subdivision - GraphNodeID: I1055"@en-AU ;
    skos:definition "209 M  Application of Subdivision"@en-AU ;
    skos:narrower C1901A00006:1054 ;
    skos:prefLabel "Item I1055"@en-AU ;
    dcat:accessURL "https://www.legislation.gov.au/C1901A00006/2024-07-01/2024-07-01/text/original/epub/OEBPS/document_3/document_3.html#_Toc172627089"^^xsd:anyURI .

C1901A00006:1056 a legcons:Item,
        skos:Concept,
        dcat:Resource ;
    rdfs:label "Item I1056"@en-AU ;
    rdfs:comment "209 N  Surrender of goods - GraphNodeID: I1056"@en-AU ;
    skos:definition "209 N  Surrender of goods"@en-AU ;
    skos:narrower C1901A00006:1054 ;
    skos:prefLabel "Item I1056"@en-AU ;
    dcat:accessURL "https://www.legislation.gov.au/C1901A00006/2024-07-01/2024-07-01/text/original/epub/OEBPS/document_3/document_3.html#_Toc172627090"^^xsd:anyURI .

C1901A00006:1057 a legcons:Item,
        skos:Concept,
        dcat:Resource ;
    rdfs:label "Item I1057"@en-AU ;
    rdfs:comment "209 P  Effect of surrender - GraphNodeID: I1057"@en-AU ;
    skos:definition "209 P  Effect of surrender"@en-AU ;
    skos:narrower C1901A00006:1054 ;
    skos:prefLabel "Item I1057"@en-AU ;
    dcat:accessURL "https://www.legislation.gov.au/C1901A00006/2024-07-01/2024-07-01/text/original/epub/OEBPS/document_3/document_3.html#_Toc172627091"^^xsd:anyURI .

C1901A00006:1058 a legcons:Item,
        skos:Concept,
        dcat:Resource ;
    rdfs:label "Item I1058"@en-AU ;
    rdfs:comment "209 Q  Right of compensation in certain circumstances for goods disposed of or destroyed - GraphNodeID: I1058"@en-AU ;
    skos:definition "209 Q  Right of compensation in certain circumstances for goods disposed of or destroyed"@en-AU ;
    skos:narrower C1901A00006:1054 ;
    skos:prefLabel "Item I1058"@en-AU ;
    dcat:accessURL "https://www.legislation.gov.au/C1901A00006/2024-07-01/2024-07-01/text/original/epub/OEBPS/document_3/document_3.html#_Toc172627092"^^xsd:anyURI .

C1901A00006:1059 a legcons:Item,
        skos:Concept,
        dcat:Resource ;
    rdfs:label "Item I1059"@en-AU ;
    rdfs:comment "209 R  Disposal of surrendered goods - GraphNodeID: I1059"@en-AU ;
    skos:definition "209 R  Disposal of surrendered goods"@en-AU ;
    skos:narrower C1901A00006:1054 ;
    skos:prefLabel "Item I1059"@en-AU ;
    dcat:accessURL "https://www.legislation.gov.au/C1901A00006/2024-07-01/2024-07-01/text/original/epub/OEBPS/document_3/document_3.html#_Toc172627093"^^xsd:anyURI .

C1901A00006:106 a legcons:Item,
        skos:Concept,
        dcat:Resource ;
    rdfs:label "Item I106"@en-AU ;
    rdfs:comment "67 EG  Special mail order house condition - GraphNodeID: I106"@en-AU ;
    skos:definition "67 EG  Special mail order house condition"@en-AU ;
    skos:narrower C1901A00006:99 ;
    skos:prefLabel "Item I106"@en-AU ;
    dcat:accessURL "https://www.legislation.gov.au/C1901A00006/2024-07-01/2024-07-01/text/original/epub/OEBPS/document_1/document_1.html#_Toc172623080"^^xsd:anyURI .

C1901A00006:1061 a legcons:Item,
        skos:Concept,
        dcat:Resource ;
    rdfs:label "Item I1061"@en-AU ;
    rdfs:comment "209 S  Definitions - GraphNodeID: I1061"@en-AU ;
    skos:definition "209 S  Definitions"@en-AU ;
    skos:narrower C1901A00006:1060 ;
    skos:prefLabel "Item I1061"@en-AU ;
    dcat:accessURL "https://www.legislation.gov.au/C1901A00006/2024-07-01/2024-07-01/text/original/epub/OEBPS/document_3/document_3.html#_Toc172627095"^^xsd:anyURI .

C1901A00006:1062 a legcons:Item,
        skos:Concept,
        dcat:Resource ;
    rdfs:label "Item I1062"@en-AU ;
    rdfs:comment "209 T  Application of Subdivision - GraphNodeID: I1062"@en-AU ;
    skos:definition "209 T  Application of Subdivision"@en-AU ;
    skos:narrower C1901A00006:1060 ;
    skos:prefLabel "Item I1062"@en-AU ;
    dcat:accessURL "https://www.legislation.gov.au/C1901A00006/2024-07-01/2024-07-01/text/original/epub/OEBPS/document_3/document_3.html#_Toc172627096"^^xsd:anyURI .

C1901A00006:1063 a legcons:Item,
        skos:Concept,
        dcat:Resource ;
    rdfs:label "Item I1063"@en-AU ;
    rdfs:comment "209 U  Power to detain goods - GraphNodeID: I1063"@en-AU ;
    skos:definition "209 U  Power to detain goods"@en-AU ;
    skos:narrower C1901A00006:1060 ;
    skos:prefLabel "Item I1063"@en-AU ;
    dcat:accessURL "https://www.legislation.gov.au/C1901A00006/2024-07-01/2024-07-01/text/original/epub/OEBPS/document_3/document_3.html#_Toc172627097"^^xsd:anyURI .

C1901A00006:1064 a legcons:Item,
        skos:Concept,
        dcat:Resource ;
    rdfs:label "Item I1064"@en-AU ;
    rdfs:comment "209 V  Detained goods to be secured - GraphNodeID: I1064"@en-AU ;
    skos:definition "209 V  Detained goods to be secured"@en-AU ;
    skos:narrower C1901A00006:1060 ;
    skos:prefLabel "Item I1064"@en-AU ;
    dcat:accessURL "https://www.legislation.gov.au/C1901A00006/2024-07-01/2024-07-01/text/original/epub/OEBPS/document_3/document_3.html#_Toc172627098"^^xsd:anyURI .

C1901A00006:1065 a legcons:Item,
        skos:Concept,
        dcat:Resource ;
    rdfs:label "Item I1065"@en-AU ;
    rdfs:comment "209 W  Requirement to serve detention notice - GraphNodeID: I1065"@en-AU ;
    skos:definition "209 W  Requirement to serve detention notice"@en-AU ;
    skos:narrower C1901A00006:1060 ;
    skos:prefLabel "Item I1065"@en-AU ;
    dcat:accessURL "https://www.legislation.gov.au/C1901A00006/2024-07-01/2024-07-01/text/original/epub/OEBPS/document_3/document_3.html#_Toc172627099"^^xsd:anyURI .

C1901A00006:1066 a legcons:Item,
        skos:Concept,
        dcat:Resource ;
    rdfs:label "Item I1066"@en-AU ;
    rdfs:comment "209 X  Matters to be dealt with in detention notices - GraphNodeID: I1066"@en-AU ;
    skos:definition "209 X  Matters to be dealt with in detention notices"@en-AU ;
    skos:narrower C1901A00006:1060 ;
    skos:prefLabel "Item I1066"@en-AU ;
    dcat:accessURL "https://www.legislation.gov.au/C1901A00006/2024-07-01/2024-07-01/text/original/epub/OEBPS/document_3/document_3.html#_Toc172627100"^^xsd:anyURI .

C1901A00006:1067 a legcons:Item,
        skos:Concept,
        dcat:Resource ;
    rdfs:label "Item I1067"@en-AU ;
    rdfs:comment "209 Y  Effect of detaining goods - GraphNodeID: I1067"@en-AU ;
    skos:definition "209 Y  Effect of detaining goods"@en-AU ;
    skos:narrower C1901A00006:1060 ;
    skos:prefLabel "Item I1067"@en-AU ;
    dcat:accessURL "https://www.legislation.gov.au/C1901A00006/2024-07-01/2024-07-01/text/original/epub/OEBPS/document_3/document_3.html#_Toc172627101"^^xsd:anyURI .

C1901A00006:1068 a legcons:Item,
        skos:Concept,
        dcat:Resource ;
    rdfs:label "Item I1068"@en-AU ;
    rdfs:comment "209 Z  Evidence not provided or permission not granted or given - GraphNodeID: I1068"@en-AU ;
    skos:definition "209 Z  Evidence not provided or permission not granted or given"@en-AU ;
    skos:narrower C1901A00006:1060 ;
    skos:prefLabel "Item I1068"@en-AU ;
    dcat:accessURL "https://www.legislation.gov.au/C1901A00006/2024-07-01/2024-07-01/text/original/epub/OEBPS/document_3/document_3.html#_Toc172627102"^^xsd:anyURI .

C1901A00006:1069 a legcons:Item,
        skos:Concept,
        dcat:Resource ;
    rdfs:label "Item I1069"@en-AU ;
    rdfs:comment "209 ZA  Evidence provided and permission granted or given - GraphNodeID: I1069"@en-AU ;
    skos:definition "209 ZA  Evidence provided and permission granted or given"@en-AU ;
    skos:narrower C1901A00006:1060 ;
    skos:prefLabel "Item I1069"@en-AU ;
    dcat:accessURL "https://www.legislation.gov.au/C1901A00006/2024-07-01/2024-07-01/text/original/epub/OEBPS/document_3/document_3.html#_Toc172627103"^^xsd:anyURI .

C1901A00006:107 a legcons:Item,
        skos:Concept,
        dcat:Resource ;
    rdfs:label "Item I107"@en-AU ;
    rdfs:comment "67 EH  Further conditions may be imposed by regulations - GraphNodeID: I107"@en-AU ;
    skos:definition "67 EH  Further conditions may be imposed by regulations"@en-AU ;
    skos:narrower C1901A00006:99 ;
    skos:prefLabel "Item I107"@en-AU ;
    dcat:accessURL "https://www.legislation.gov.au/C1901A00006/2024-07-01/2024-07-01/text/original/epub/OEBPS/document_1/document_1.html#_Toc172623081"^^xsd:anyURI .

C1901A00006:1070 a legcons:Item,
        skos:Concept,
        dcat:Resource ;
    rdfs:label "Item I1070"@en-AU ;
    rdfs:comment "209 ZB  Service by post - GraphNodeID: I1070"@en-AU ;
    skos:definition "209 ZB  Service by post"@en-AU ;
    skos:narrower C1901A00006:1060 ;
    skos:prefLabel "Item I1070"@en-AU ;
    dcat:accessURL "https://www.legislation.gov.au/C1901A00006/2024-07-01/2024-07-01/text/original/epub/OEBPS/document_3/document_3.html#_Toc172627104"^^xsd:anyURI .

C1901A00006:1071 a legcons:Item,
        skos:Concept,
        dcat:Resource ;
    rdfs:label "Item I1071"@en-AU ;
    rdfs:comment "209 ZC  Liability for detention of goods - GraphNodeID: I1071"@en-AU ;
    skos:definition "209 ZC  Liability for detention of goods"@en-AU ;
    skos:narrower C1901A00006:1060 ;
    skos:prefLabel "Item I1071"@en-AU ;
    dcat:accessURL "https://www.legislation.gov.au/C1901A00006/2024-07-01/2024-07-01/text/original/epub/OEBPS/document_3/document_3.html#_Toc172627105"^^xsd:anyURI .

C1901A00006:1073 a legcons:Item,
        skos:Concept,
        dcat:Resource ;
    rdfs:label "Item I1073"@en-AU ;
    rdfs:comment "210  Power of arrest without warrant - GraphNodeID: I1073"@en-AU ;
    skos:definition "210  Power of arrest without warrant"@en-AU ;
    skos:narrower C1901A00006:1072 ;
    skos:prefLabel "Item I1073"@en-AU ;
    dcat:accessURL "https://www.legislation.gov.au/C1901A00006/2024-07-01/2024-07-01/text/original/epub/OEBPS/document_3/document_3.html#_Toc172627107"^^xsd:anyURI .

C1901A00006:1074 a legcons:Item,
        skos:Concept,
        dcat:Resource ;
    rdfs:label "Item I1074"@en-AU ;
    rdfs:comment "210 A  Use of force in making arrest - GraphNodeID: I1074"@en-AU ;
    skos:definition "210 A  Use of force in making arrest"@en-AU ;
    skos:narrower C1901A00006:1072 ;
    skos:prefLabel "Item I1074"@en-AU ;
    dcat:accessURL "https://www.legislation.gov.au/C1901A00006/2024-07-01/2024-07-01/text/original/epub/OEBPS/document_3/document_3.html#_Toc172627108"^^xsd:anyURI .

C1901A00006:1075 a legcons:Item,
        skos:Concept,
        dcat:Resource ;
    rdfs:label "Item I1075"@en-AU ;
    rdfs:comment "210 B  Person to be informed of grounds of arrest - GraphNodeID: I1075"@en-AU ;
    skos:definition "210 B  Person to be informed of grounds of arrest"@en-AU ;
    skos:narrower C1901A00006:1072 ;
    skos:prefLabel "Item I1075"@en-AU ;
    dcat:accessURL "https://www.legislation.gov.au/C1901A00006/2024-07-01/2024-07-01/text/original/epub/OEBPS/document_3/document_3.html#_Toc172627109"^^xsd:anyURI .

C1901A00006:1076 a legcons:Item,
        skos:Concept,
        dcat:Resource ;
    rdfs:label "Item I1076"@en-AU ;
    rdfs:comment "211  Power to conduct a frisk search of an arrested person - GraphNodeID: I1076"@en-AU ;
    skos:definition "211  Power to conduct a frisk search of an arrested person"@en-AU ;
    skos:narrower C1901A00006:1072 ;
    skos:prefLabel "Item I1076"@en-AU ;
    dcat:accessURL "https://www.legislation.gov.au/C1901A00006/2024-07-01/2024-07-01/text/original/epub/OEBPS/document_3/document_3.html#_Toc172627110"^^xsd:anyURI .

C1901A00006:1077 a legcons:Item,
        skos:Concept,
        dcat:Resource ;
    rdfs:label "Item I1077"@en-AU ;
    rdfs:comment "211 A  Power to conduct an ordinary search of an arrested person - GraphNodeID: I1077"@en-AU ;
    skos:definition "211 A  Power to conduct an ordinary search of an arrested person"@en-AU ;
    skos:narrower C1901A00006:1072 ;
    skos:prefLabel "Item I1077"@en-AU ;
    dcat:accessURL "https://www.legislation.gov.au/C1901A00006/2024-07-01/2024-07-01/text/original/epub/OEBPS/document_3/document_3.html#_Toc172627111"^^xsd:anyURI .

C1901A00006:1078 a legcons:Item,
        skos:Concept,
        dcat:Resource ;
    rdfs:label "Item I1078"@en-AU ;
    rdfs:comment "212  How arrested person to be dealt with - GraphNodeID: I1078"@en-AU ;
    skos:definition "212  How arrested person to be dealt with"@en-AU ;
    skos:narrower C1901A00006:1072 ;
    skos:prefLabel "Item I1078"@en-AU ;
    dcat:accessURL "https://www.legislation.gov.au/C1901A00006/2024-07-01/2024-07-01/text/original/epub/OEBPS/document_3/document_3.html#_Toc172627112"^^xsd:anyURI .

C1901A00006:1079 a legcons:Item,
        skos:Concept,
        dcat:Resource ;
    rdfs:label "Item I1079"@en-AU ;
    rdfs:comment "213  Requirement to provide name etc - GraphNodeID: I1079"@en-AU ;
    skos:definition "213  Requirement to provide name etc"@en-AU ;
    skos:narrower C1901A00006:1072 ;
    skos:prefLabel "Item I1079"@en-AU ;
    dcat:accessURL "https://www.legislation.gov.au/C1901A00006/2024-07-01/2024-07-01/text/original/epub/OEBPS/document_3/document_3.html#_Toc172627113"^^xsd:anyURI .

C1901A00006:108 a legcons:Item,
        skos:Concept,
        dcat:Resource ;
    rdfs:label "Item I108"@en-AU ;
    rdfs:comment "67 EI  Breach of conditions of registration - GraphNodeID: I108"@en-AU ;
    skos:definition "67 EI  Breach of conditions of registration"@en-AU ;
    skos:narrower C1901A00006:99 ;
    skos:prefLabel "Item I108"@en-AU ;
    dcat:accessURL "https://www.legislation.gov.au/C1901A00006/2024-07-01/2024-07-01/text/original/epub/OEBPS/document_1/document_1.html#_Toc172623082"^^xsd:anyURI .

C1901A00006:1081 a legcons:Item,
        skos:Concept,
        dcat:Resource ;
    rdfs:label "Item I1081"@en-AU ;
    rdfs:comment "213 A  Providing an authorised officer with information about people working in restricted areas - GraphNodeID: I1081"@en-AU ;
    skos:definition "213 A  Providing an authorised officer with information about people working in restricted areas"@en-AU ;
    skos:narrower C1901A00006:1080 ;
    skos:prefLabel "Item I1081"@en-AU ;
    dcat:accessURL "https://www.legislation.gov.au/C1901A00006/2024-07-01/2024-07-01/text/original/epub/OEBPS/document_3/document_3.html#_Toc172627115"^^xsd:anyURI .

C1901A00006:1082 a legcons:Item,
        skos:Concept,
        dcat:Resource ;
    rdfs:label "Item I1082"@en-AU ;
    rdfs:comment "213 B  Provision of information about people issued with security identification cards - GraphNodeID: I1082"@en-AU ;
    skos:definition "213 B  Provision of information about people issued with security identification cards"@en-AU ;
    skos:narrower C1901A00006:1080 ;
    skos:prefLabel "Item I1082"@en-AU ;
    dcat:accessURL "https://www.legislation.gov.au/C1901A00006/2024-07-01/2024-07-01/text/original/epub/OEBPS/document_3/document_3.html#_Toc172627116"^^xsd:anyURI .

C1901A00006:1084 a legcons:Item,
        skos:Concept,
        dcat:Resource ;
    rdfs:label "Item I1084"@en-AU ;
    rdfs:comment "214 AA  Occupier of premises - GraphNodeID: I1084"@en-AU ;
    skos:definition "214 AA  Occupier of premises"@en-AU ;
    skos:narrower C1901A00006:1083 ;
    skos:prefLabel "Item I1084"@en-AU ;
    dcat:accessURL "https://www.legislation.gov.au/C1901A00006/2024-07-01/2024-07-01/text/original/epub/OEBPS/document_3/document_3.html#_Toc172627118"^^xsd:anyURI .

C1901A00006:1085 a legcons:Item,
        skos:Concept,
        dcat:Resource ;
    rdfs:label "Item I1085"@en-AU ;
    rdfs:comment "214 AB  What are monitoring powers - GraphNodeID: I1085"@en-AU ;
    skos:definition "214 AB  What are monitoring powers"@en-AU ;
    skos:narrower C1901A00006:1083 ;
    skos:prefLabel "Item I1085"@en-AU ;
    dcat:accessURL "https://www.legislation.gov.au/C1901A00006/2024-07-01/2024-07-01/text/original/epub/OEBPS/document_3/document_3.html#_Toc172627119"^^xsd:anyURI .

C1901A00006:1086 a legcons:Item,
        skos:Concept,
        dcat:Resource ;
    rdfs:label "Item I1086"@en-AU ;
    rdfs:comment "214 AC  Monitoring officers - GraphNodeID: I1086"@en-AU ;
    skos:definition "214 AC  Monitoring officers"@en-AU ;
    skos:narrower C1901A00006:1083 ;
    skos:prefLabel "Item I1086"@en-AU ;
    dcat:accessURL "https://www.legislation.gov.au/C1901A00006/2024-07-01/2024-07-01/text/original/epub/OEBPS/document_3/document_3.html#_Toc172627120"^^xsd:anyURI .

C1901A00006:1087 a legcons:Item,
        skos:Concept,
        dcat:Resource ;
    rdfs:label "Item I1087"@en-AU ;
    rdfs:comment "214 ACA  Monitoring officer to notify occupier of premises of the occupiers rights and obligations - GraphNodeID: I1087"@en-AU ;
    skos:definition "214 ACA  Monitoring officer to notify occupier of premises of the occupiers rights and obligations"@en-AU ;
    skos:narrower C1901A00006:1083 ;
    skos:prefLabel "Item I1087"@en-AU ;
    dcat:accessURL "https://www.legislation.gov.au/C1901A00006/2024-07-01/2024-07-01/text/original/epub/OEBPS/document_3/document_3.html#_Toc172627121"^^xsd:anyURI .

C1901A00006:1088 a legcons:Item,
        skos:Concept,
        dcat:Resource ;
    rdfs:label "Item I1088"@en-AU ;
    rdfs:comment "214 AD  Notice of proposal to exercise monitoring powers - GraphNodeID: I1088"@en-AU ;
    skos:definition "214 AD  Notice of proposal to exercise monitoring powers"@en-AU ;
    skos:narrower C1901A00006:1083 ;
    skos:prefLabel "Item I1088"@en-AU ;
    dcat:accessURL "https://www.legislation.gov.au/C1901A00006/2024-07-01/2024-07-01/text/original/epub/OEBPS/document_3/document_3.html#_Toc172627122"^^xsd:anyURI .

C1901A00006:1089 a legcons:Item,
        skos:Concept,
        dcat:Resource ;
    rdfs:label "Item I1089"@en-AU ;
    rdfs:comment "214 AE  Exercise of monitoring powers with consent - GraphNodeID: I1089"@en-AU ;
    skos:definition "214 AE  Exercise of monitoring powers with consent"@en-AU ;
    skos:narrower C1901A00006:1083 ;
    skos:prefLabel "Item I1089"@en-AU ;
    dcat:accessURL "https://www.legislation.gov.au/C1901A00006/2024-07-01/2024-07-01/text/original/epub/OEBPS/document_3/document_3.html#_Toc172627123"^^xsd:anyURI .

C1901A00006:109 a legcons:Item,
        skos:Concept,
        dcat:Resource ;
    rdfs:label "Item I109"@en-AU ;
    rdfs:comment "67 EJ  Duration of registration - GraphNodeID: I109"@en-AU ;
    skos:definition "67 EJ  Duration of registration"@en-AU ;
    skos:narrower C1901A00006:99 ;
    skos:prefLabel "Item I109"@en-AU ;
    dcat:accessURL "https://www.legislation.gov.au/C1901A00006/2024-07-01/2024-07-01/text/original/epub/OEBPS/document_1/document_1.html#_Toc172623083"^^xsd:anyURI .

C1901A00006:1090 a legcons:Item,
        skos:Concept,
        dcat:Resource ;
    rdfs:label "Item I1090"@en-AU ;
    rdfs:comment "214 AF  Exercise of monitoring powers under a warrant - GraphNodeID: I1090"@en-AU ;
    skos:definition "214 AF  Exercise of monitoring powers under a warrant"@en-AU ;
    skos:narrower C1901A00006:1083 ;
    skos:prefLabel "Item I1090"@en-AU ;
    dcat:accessURL "https://www.legislation.gov.au/C1901A00006/2024-07-01/2024-07-01/text/original/epub/OEBPS/document_3/document_3.html#_Toc172627124"^^xsd:anyURI .

C1901A00006:1091 a legcons:Item,
        skos:Concept,
        dcat:Resource ;
    rdfs:label "Item I1091"@en-AU ;
    rdfs:comment "214 AG  Warrants may be granted by telephone or other electronic means - GraphNodeID: I1091"@en-AU ;
    skos:definition "214 AG  Warrants may be granted by telephone or other electronic means"@en-AU ;
    skos:narrower C1901A00006:1083 ;
    skos:prefLabel "Item I1091"@en-AU ;
    dcat:accessURL "https://www.legislation.gov.au/C1901A00006/2024-07-01/2024-07-01/text/original/epub/OEBPS/document_3/document_3.html#_Toc172627125"^^xsd:anyURI .

C1901A00006:1092 a legcons:Item,
        skos:Concept,
        dcat:Resource ;
    rdfs:label "Item I1092"@en-AU ;
    rdfs:comment "214 AH  Monitoring officer may ask questions - GraphNodeID: I1092"@en-AU ;
    skos:definition "214 AH  Monitoring officer may ask questions"@en-AU ;
    skos:narrower C1901A00006:1083 ;
    skos:prefLabel "Item I1092"@en-AU ;
    dcat:accessURL "https://www.legislation.gov.au/C1901A00006/2024-07-01/2024-07-01/text/original/epub/OEBPS/document_3/document_3.html#_Toc172627126"^^xsd:anyURI .

C1901A00006:1093 a legcons:Item,
        skos:Concept,
        dcat:Resource ;
    rdfs:label "Item I1093"@en-AU ;
    rdfs:comment "214 AI  Monitoring officer may ask for assistance - GraphNodeID: I1093"@en-AU ;
    skos:definition "214 AI  Monitoring officer may ask for assistance"@en-AU ;
    skos:narrower C1901A00006:1083 ;
    skos:prefLabel "Item I1093"@en-AU ;
    dcat:accessURL "https://www.legislation.gov.au/C1901A00006/2024-07-01/2024-07-01/text/original/epub/OEBPS/document_3/document_3.html#_Toc172627127"^^xsd:anyURI .

C1901A00006:1094 a legcons:Item,
        skos:Concept,
        dcat:Resource ;
    rdfs:label "Item I1094"@en-AU ;
    rdfs:comment "214 AJ  Compensation for damage to electronic equipment - GraphNodeID: I1094"@en-AU ;
    skos:definition "214 AJ  Compensation for damage to electronic equipment"@en-AU ;
    skos:narrower C1901A00006:1083 ;
    skos:prefLabel "Item I1094"@en-AU ;
    dcat:accessURL "https://www.legislation.gov.au/C1901A00006/2024-07-01/2024-07-01/text/original/epub/OEBPS/document_3/document_3.html#_Toc172627128"^^xsd:anyURI .

C1901A00006:1095 a legcons:Item,
        skos:Concept,
        dcat:Resource ;
    rdfs:label "Item I1095"@en-AU ;
    rdfs:comment "214 B  Powers of officers for purposes of Customs Tariff Anti Dumping Act 1975 - GraphNodeID: I1095"@en-AU ;
    skos:definition "214 B  Powers of officers for purposes of Customs Tariff Anti Dumping Act 1975"@en-AU ;
    skos:narrower C1901A00006:1083 ;
    skos:prefLabel "Item I1095"@en-AU ;
    dcat:accessURL "https://www.legislation.gov.au/C1901A00006/2024-07-01/2024-07-01/text/original/epub/OEBPS/document_3/document_3.html#_Toc172627129"^^xsd:anyURI .

C1901A00006:1097 a legcons:Item,
        skos:Concept,
        dcat:Resource ;
    rdfs:label "Item I1097"@en-AU ;
    rdfs:comment "214 BAA  Simplified outline - GraphNodeID: I1097"@en-AU ;
    skos:definition "214 BAA  Simplified outline"@en-AU ;
    skos:narrower C1901A00006:1096 ;
    skos:prefLabel "Item I1097"@en-AU ;
    dcat:accessURL "https://www.legislation.gov.au/C1901A00006/2024-07-01/2024-07-01/text/original/epub/OEBPS/document_3/document_3.html#_Toc172627131"^^xsd:anyURI .

C1901A00006:1098 a legcons:Item,
        skos:Concept,
        dcat:Resource ;
    rdfs:label "Item I1098"@en-AU ;
    rdfs:comment "214 BAB  Definitions - GraphNodeID: I1098"@en-AU ;
    skos:definition "214 BAB  Definitions"@en-AU ;
    skos:narrower C1901A00006:1096 ;
    skos:prefLabel "Item I1098"@en-AU ;
    dcat:accessURL "https://www.legislation.gov.au/C1901A00006/2024-07-01/2024-07-01/text/original/epub/OEBPS/document_3/document_3.html#_Toc172627132"^^xsd:anyURI .

C1901A00006:1099 a legcons:Item,
        skos:Concept,
        dcat:Resource ;
    rdfs:label "Item I1099"@en-AU ;
    rdfs:comment "214 BAC  AUSFTA verification powers - GraphNodeID: I1099"@en-AU ;
    skos:definition "214 BAC  AUSFTA verification powers"@en-AU ;
    skos:narrower C1901A00006:1096 ;
    skos:prefLabel "Item I1099"@en-AU ;
    dcat:accessURL "https://www.legislation.gov.au/C1901A00006/2024-07-01/2024-07-01/text/original/epub/OEBPS/document_3/document_3.html#_Toc172627133"^^xsd:anyURI .

C1901A00006:11 a legcons:Item,
        skos:Concept,
        dcat:Resource ;
    rdfs:label "Item I11"@en-AU ;
    rdfs:comment "4 C  Identity cards - GraphNodeID: I11"@en-AU ;
    skos:definition "4 C  Identity cards"@en-AU ;
    skos:narrower C1901A00006:2 ;
    skos:prefLabel "Item I11"@en-AU ;
    dcat:accessURL "https://www.legislation.gov.au/C1901A00006/2024-07-01/2024-07-01/text/original/epub/OEBPS/document_1/document_1.html#_Toc172622985"^^xsd:anyURI .

C1901A00006:110 a legcons:Item,
        skos:Concept,
        dcat:Resource ;
    rdfs:label "Item I110"@en-AU ;
    rdfs:comment "67 EK  Renewal of registration - GraphNodeID: I110"@en-AU ;
    skos:definition "67 EK  Renewal of registration"@en-AU ;
    skos:narrower C1901A00006:99 ;
    skos:prefLabel "Item I110"@en-AU ;
    dcat:accessURL "https://www.legislation.gov.au/C1901A00006/2024-07-01/2024-07-01/text/original/epub/OEBPS/document_1/document_1.html#_Toc172623084"^^xsd:anyURI .

C1901A00006:1100 a legcons:Item,
        skos:Concept,
        dcat:Resource ;
    rdfs:label "Item I1100"@en-AU ;
    rdfs:comment "214 BAD  Appointment of verification officers - GraphNodeID: I1100"@en-AU ;
    skos:definition "214 BAD  Appointment of verification officers"@en-AU ;
    skos:narrower C1901A00006:1096 ;
    skos:prefLabel "Item I1100"@en-AU ;
    dcat:accessURL "https://www.legislation.gov.au/C1901A00006/2024-07-01/2024-07-01/text/original/epub/OEBPS/document_3/document_3.html#_Toc172627134"^^xsd:anyURI .

C1901A00006:1101 a legcons:Item,
        skos:Concept,
        dcat:Resource ;
    rdfs:label "Item I1101"@en-AU ;
    rdfs:comment "214 BAE  Verification officers may enter premises and exercise AUSFTA verification powers with consent - GraphNodeID: I1101"@en-AU ;
    skos:definition "214 BAE  Verification officers may enter premises and exercise AUSFTA verification powers with consent"@en-AU ;
    skos:narrower C1901A00006:1096 ;
    skos:prefLabel "Item I1101"@en-AU ;
    dcat:accessURL "https://www.legislation.gov.au/C1901A00006/2024-07-01/2024-07-01/text/original/epub/OEBPS/document_3/document_3.html#_Toc172627135"^^xsd:anyURI .

C1901A00006:1102 a legcons:Item,
        skos:Concept,
        dcat:Resource ;
    rdfs:label "Item I1102"@en-AU ;
    rdfs:comment "214 BAF  US customs officials may accompany verification officers - GraphNodeID: I1102"@en-AU ;
    skos:definition "214 BAF  US customs officials may accompany verification officers"@en-AU ;
    skos:narrower C1901A00006:1096 ;
    skos:prefLabel "Item I1102"@en-AU ;
    dcat:accessURL "https://www.legislation.gov.au/C1901A00006/2024-07-01/2024-07-01/text/original/epub/OEBPS/document_3/document_3.html#_Toc172627136"^^xsd:anyURI .

C1901A00006:1103 a legcons:Item,
        skos:Concept,
        dcat:Resource ;
    rdfs:label "Item I1103"@en-AU ;
    rdfs:comment "214 BAG  Availability of assistance in exercising AUSFTA verification powers - GraphNodeID: I1103"@en-AU ;
    skos:definition "214 BAG  Availability of assistance in exercising AUSFTA verification powers"@en-AU ;
    skos:narrower C1901A00006:1096 ;
    skos:prefLabel "Item I1103"@en-AU ;
    dcat:accessURL "https://www.legislation.gov.au/C1901A00006/2024-07-01/2024-07-01/text/original/epub/OEBPS/document_3/document_3.html#_Toc172627137"^^xsd:anyURI .

C1901A00006:1104 a legcons:Item,
        skos:Concept,
        dcat:Resource ;
    rdfs:label "Item I1104"@en-AU ;
    rdfs:comment "214 BAH  Verification officer may ask questions - GraphNodeID: I1104"@en-AU ;
    skos:definition "214 BAH  Verification officer may ask questions"@en-AU ;
    skos:narrower C1901A00006:1096 ;
    skos:prefLabel "Item I1104"@en-AU ;
    dcat:accessURL "https://www.legislation.gov.au/C1901A00006/2024-07-01/2024-07-01/text/original/epub/OEBPS/document_3/document_3.html#_Toc172627138"^^xsd:anyURI .

C1901A00006:1105 a legcons:Item,
        skos:Concept,
        dcat:Resource ;
    rdfs:label "Item I1105"@en-AU ;
    rdfs:comment "214 BAI  Verification officer may ask for assistance - GraphNodeID: I1105"@en-AU ;
    skos:definition "214 BAI  Verification officer may ask for assistance"@en-AU ;
    skos:narrower C1901A00006:1096 ;
    skos:prefLabel "Item I1105"@en-AU ;
    dcat:accessURL "https://www.legislation.gov.au/C1901A00006/2024-07-01/2024-07-01/text/original/epub/OEBPS/document_3/document_3.html#_Toc172627139"^^xsd:anyURI .

C1901A00006:1106 a legcons:Item,
        skos:Concept,
        dcat:Resource ;
    rdfs:label "Item I1106"@en-AU ;
    rdfs:comment "214 BAJ  Verification officer may disclose information to US - GraphNodeID: I1106"@en-AU ;
    skos:definition "214 BAJ  Verification officer may disclose information to US"@en-AU ;
    skos:narrower C1901A00006:1096 ;
    skos:prefLabel "Item I1106"@en-AU ;
    dcat:accessURL "https://www.legislation.gov.au/C1901A00006/2024-07-01/2024-07-01/text/original/epub/OEBPS/document_3/document_3.html#_Toc172627140"^^xsd:anyURI .

C1901A00006:1107 a legcons:Item,
        skos:Concept,
        dcat:Resource ;
    rdfs:label "Item I1107"@en-AU ;
    rdfs:comment "214 BAK  Operation of electronic equipment at premises - GraphNodeID: I1107"@en-AU ;
    skos:definition "214 BAK  Operation of electronic equipment at premises"@en-AU ;
    skos:narrower C1901A00006:1096 ;
    skos:prefLabel "Item I1107"@en-AU ;
    dcat:accessURL "https://www.legislation.gov.au/C1901A00006/2024-07-01/2024-07-01/text/original/epub/OEBPS/document_3/document_3.html#_Toc172627141"^^xsd:anyURI .

C1901A00006:1108 a legcons:Item,
        skos:Concept,
        dcat:Resource ;
    rdfs:label "Item I1108"@en-AU ;
    rdfs:comment "214 BAL  Compensation for damage to electronic equipment - GraphNodeID: I1108"@en-AU ;
    skos:definition "214 BAL  Compensation for damage to electronic equipment"@en-AU ;
    skos:narrower C1901A00006:1096 ;
    skos:prefLabel "Item I1108"@en-AU ;
    dcat:accessURL "https://www.legislation.gov.au/C1901A00006/2024-07-01/2024-07-01/text/original/epub/OEBPS/document_3/document_3.html#_Toc172627142"^^xsd:anyURI .

C1901A00006:111 a legcons:Item,
        skos:Concept,
        dcat:Resource ;
    rdfs:label "Item I111"@en-AU ;
    rdfs:comment "67 EL  Comptroller General of Customs to allocate a special identifying code for each special reporter - GraphNodeID: I111"@en-AU ;
    skos:definition "67 EL  Comptroller General of Customs to allocate a special identifying code for each special reporter"@en-AU ;
    skos:narrower C1901A00006:99 ;
    skos:prefLabel "Item I111"@en-AU ;
    dcat:accessURL "https://www.legislation.gov.au/C1901A00006/2024-07-01/2024-07-01/text/original/epub/OEBPS/document_1/document_1.html#_Toc172623085"^^xsd:anyURI .

C1901A00006:1110 a legcons:Item,
        skos:Concept,
        dcat:Resource ;
    rdfs:label "Item I1110"@en-AU ;
    rdfs:comment "214 BA  Nature of functions of magistrate under sections 203 S and 205 E - GraphNodeID: I1110"@en-AU ;
    skos:definition "214 BA  Nature of functions of magistrate under sections 203 S and 205 E"@en-AU ;
    skos:narrower C1901A00006:1109 ;
    skos:prefLabel "Item I1110"@en-AU ;
    dcat:accessURL "https://www.legislation.gov.au/C1901A00006/2024-07-01/2024-07-01/text/original/epub/OEBPS/document_3/document_3.html#_Toc172627144"^^xsd:anyURI .

C1901A00006:1111 a legcons:Item,
        skos:Concept,
        dcat:Resource ;
    rdfs:label "Item I1111"@en-AU ;
    rdfs:comment "215  Collector may impound documents - GraphNodeID: I1111"@en-AU ;
    skos:definition "215  Collector may impound documents"@en-AU ;
    skos:narrower C1901A00006:1109 ;
    skos:prefLabel "Item I1111"@en-AU ;
    dcat:accessURL "https://www.legislation.gov.au/C1901A00006/2024-07-01/2024-07-01/text/original/epub/OEBPS/document_3/document_3.html#_Toc172627145"^^xsd:anyURI .

C1901A00006:1112 a legcons:Item,
        skos:Concept,
        dcat:Resource ;
    rdfs:label "Item I1112"@en-AU ;
    rdfs:comment "217  Translations of foreign invoices - GraphNodeID: I1112"@en-AU ;
    skos:definition "217  Translations of foreign invoices"@en-AU ;
    skos:narrower C1901A00006:1109 ;
    skos:prefLabel "Item I1112"@en-AU ;
    dcat:accessURL "https://www.legislation.gov.au/C1901A00006/2024-07-01/2024-07-01/text/original/epub/OEBPS/document_3/document_3.html#_Toc172627146"^^xsd:anyURI .

C1901A00006:1113 a legcons:Item,
        skos:Concept,
        dcat:Resource ;
    rdfs:label "Item I1113"@en-AU ;
    rdfs:comment "218  Samples - GraphNodeID: I1113"@en-AU ;
    skos:definition "218  Samples"@en-AU ;
    skos:narrower C1901A00006:1109 ;
    skos:prefLabel "Item I1113"@en-AU ;
    dcat:accessURL "https://www.legislation.gov.au/C1901A00006/2024-07-01/2024-07-01/text/original/epub/OEBPS/document_3/document_3.html#_Toc172627147"^^xsd:anyURI .

C1901A00006:1114 a legcons:Item,
        skos:Concept,
        dcat:Resource ;
    rdfs:label "Item I1114"@en-AU ;
    rdfs:comment "218 A  Disposal of certain abandoned goods - GraphNodeID: I1114"@en-AU ;
    skos:definition "218 A  Disposal of certain abandoned goods"@en-AU ;
    skos:narrower C1901A00006:1109 ;
    skos:prefLabel "Item I1114"@en-AU ;
    dcat:accessURL "https://www.legislation.gov.au/C1901A00006/2024-07-01/2024-07-01/text/original/epub/OEBPS/document_3/document_3.html#_Toc172627148"^^xsd:anyURI .

C1901A00006:1117 a legcons:Item,
        skos:Concept,
        dcat:Resource ;
    rdfs:label "Item I1117"@en-AU ;
    rdfs:comment "219 L  Detention for frisk search - GraphNodeID: I1117"@en-AU ;
    skos:definition "219 L  Detention for frisk search"@en-AU ;
    skos:narrower C1901A00006:1116 ;
    skos:prefLabel "Item I1117"@en-AU ;
    dcat:accessURL "https://www.legislation.gov.au/C1901A00006/2024-07-01/2024-07-01/text/original/epub/OEBPS/document_3/document_3.html#_Toc172627151"^^xsd:anyURI .

C1901A00006:1118 a legcons:Item,
        skos:Concept,
        dcat:Resource ;
    rdfs:label "Item I1118"@en-AU ;
    rdfs:comment "219 M  Frisk search - GraphNodeID: I1118"@en-AU ;
    skos:definition "219 M  Frisk search"@en-AU ;
    skos:narrower C1901A00006:1116 ;
    skos:prefLabel "Item I1118"@en-AU ;
    dcat:accessURL "https://www.legislation.gov.au/C1901A00006/2024-07-01/2024-07-01/text/original/epub/OEBPS/document_3/document_3.html#_Toc172627152"^^xsd:anyURI .

C1901A00006:1119 a legcons:Item,
        skos:Concept,
        dcat:Resource ;
    rdfs:label "Item I1119"@en-AU ;
    rdfs:comment "219 N  Power to require the production of things - GraphNodeID: I1119"@en-AU ;
    skos:definition "219 N  Power to require the production of things"@en-AU ;
    skos:narrower C1901A00006:1116 ;
    skos:prefLabel "Item I1119"@en-AU ;
    dcat:accessURL "https://www.legislation.gov.au/C1901A00006/2024-07-01/2024-07-01/text/original/epub/OEBPS/document_3/document_3.html#_Toc172627153"^^xsd:anyURI .

C1901A00006:112 a legcons:Item,
        skos:Concept,
        dcat:Resource ;
    rdfs:label "Item I112"@en-AU ;
    rdfs:comment "67 EM  Cancellation of registration as special reporter - GraphNodeID: I112"@en-AU ;
    skos:definition "67 EM  Cancellation of registration as special reporter"@en-AU ;
    skos:narrower C1901A00006:99 ;
    skos:prefLabel "Item I112"@en-AU ;
    dcat:accessURL "https://www.legislation.gov.au/C1901A00006/2024-07-01/2024-07-01/text/original/epub/OEBPS/document_1/document_1.html#_Toc172623086"^^xsd:anyURI .

C1901A00006:1120 a legcons:Item,
        skos:Concept,
        dcat:Resource ;
    rdfs:label "Item I1120"@en-AU ;
    rdfs:comment "219 P  Persons to whom section 219 R applies - GraphNodeID: I1120"@en-AU ;
    skos:definition "219 P  Persons to whom section 219 R applies"@en-AU ;
    skos:narrower C1901A00006:1116 ;
    skos:prefLabel "Item I1120"@en-AU ;
    dcat:accessURL "https://www.legislation.gov.au/C1901A00006/2024-07-01/2024-07-01/text/original/epub/OEBPS/document_3/document_3.html#_Toc172627154"^^xsd:anyURI .

C1901A00006:1122 a legcons:Item,
        skos:Concept,
        dcat:Resource ;
    rdfs:label "Item I1122"@en-AU ;
    rdfs:comment "219 Q  Detention for external search - GraphNodeID: I1122"@en-AU ;
    skos:definition "219 Q  Detention for external search"@en-AU ;
    skos:narrower C1901A00006:1121 ;
    skos:prefLabel "Item I1122"@en-AU ;
    dcat:accessURL "https://www.legislation.gov.au/C1901A00006/2024-07-01/2024-07-01/text/original/epub/OEBPS/document_3/document_3.html#_Toc172627156"^^xsd:anyURI .

C1901A00006:1123 a legcons:Item,
        skos:Concept,
        dcat:Resource ;
    rdfs:label "Item I1123"@en-AU ;
    rdfs:comment "219 R  External search - GraphNodeID: I1123"@en-AU ;
    skos:definition "219 R  External search"@en-AU ;
    skos:narrower C1901A00006:1121 ;
    skos:prefLabel "Item I1123"@en-AU ;
    dcat:accessURL "https://www.legislation.gov.au/C1901A00006/2024-07-01/2024-07-01/text/original/epub/OEBPS/document_3/document_3.html#_Toc172627157"^^xsd:anyURI .

C1901A00006:1124 a legcons:Item,
        skos:Concept,
        dcat:Resource ;
    rdfs:label "Item I1124"@en-AU ;
    rdfs:comment "219 RAA  Videotape record may be made of external search - GraphNodeID: I1124"@en-AU ;
    skos:definition "219 RAA  Videotape record may be made of external search"@en-AU ;
    skos:narrower C1901A00006:1121 ;
    skos:prefLabel "Item I1124"@en-AU ;
    dcat:accessURL "https://www.legislation.gov.au/C1901A00006/2024-07-01/2024-07-01/text/original/epub/OEBPS/document_3/document_3.html#_Toc172627158"^^xsd:anyURI .

C1901A00006:1126 a legcons:Item,
        skos:Concept,
        dcat:Resource ;
    rdfs:label "Item I1126"@en-AU ;
    rdfs:comment "219 RA  Certain Judges and Magistrates eligible to give orders under this Subdivision - GraphNodeID: I1126"@en-AU ;
    skos:definition "219 RA  Certain Judges and Magistrates eligible to give orders under this Subdivision"@en-AU ;
    skos:narrower C1901A00006:1125 ;
    skos:prefLabel "Item I1126"@en-AU ;
    dcat:accessURL "https://www.legislation.gov.au/C1901A00006/2024-07-01/2024-07-01/text/original/epub/OEBPS/document_3/document_3.html#_Toc172627160"^^xsd:anyURI .

C1901A00006:1127 a legcons:Item,
        skos:Concept,
        dcat:Resource ;
    rdfs:label "Item I1127"@en-AU ;
    rdfs:comment "219 S  Initial detention - GraphNodeID: I1127"@en-AU ;
    skos:definition "219 S  Initial detention"@en-AU ;
    skos:narrower C1901A00006:1125 ;
    skos:prefLabel "Item I1127"@en-AU ;
    dcat:accessURL "https://www.legislation.gov.au/C1901A00006/2024-07-01/2024-07-01/text/original/epub/OEBPS/document_3/document_3.html#_Toc172627161"^^xsd:anyURI .

C1901A00006:1128 a legcons:Item,
        skos:Concept,
        dcat:Resource ;
    rdfs:label "Item I1128"@en-AU ;
    rdfs:comment "219 SA  Internal non medical scan using prescribed equipment - GraphNodeID: I1128"@en-AU ;
    skos:definition "219 SA  Internal non medical scan using prescribed equipment"@en-AU ;
    skos:narrower C1901A00006:1125 ;
    skos:prefLabel "Item I1128"@en-AU ;
    dcat:accessURL "https://www.legislation.gov.au/C1901A00006/2024-07-01/2024-07-01/text/original/epub/OEBPS/document_3/document_3.html#_Toc172627162"^^xsd:anyURI .

C1901A00006:1129 a legcons:Item,
        skos:Concept,
        dcat:Resource ;
    rdfs:label "Item I1129"@en-AU ;
    rdfs:comment "219 SB  Seeking detention order following invitation to consent to internal non medical scan - GraphNodeID: I1129"@en-AU ;
    skos:definition "219 SB  Seeking detention order following invitation to consent to internal non medical scan"@en-AU ;
    skos:narrower C1901A00006:1125 ;
    skos:prefLabel "Item I1129"@en-AU ;
    dcat:accessURL "https://www.legislation.gov.au/C1901A00006/2024-07-01/2024-07-01/text/original/epub/OEBPS/document_3/document_3.html#_Toc172627163"^^xsd:anyURI .

C1901A00006:1130 a legcons:Item,
        skos:Concept,
        dcat:Resource ;
    rdfs:label "Item I1130"@en-AU ;
    rdfs:comment "219 T  Initial order for detention - GraphNodeID: I1130"@en-AU ;
    skos:definition "219 T  Initial order for detention"@en-AU ;
    skos:narrower C1901A00006:1125 ;
    skos:prefLabel "Item I1130"@en-AU ;
    dcat:accessURL "https://www.legislation.gov.au/C1901A00006/2024-07-01/2024-07-01/text/original/epub/OEBPS/document_3/document_3.html#_Toc172627164"^^xsd:anyURI .

C1901A00006:1131 a legcons:Item,
        skos:Concept,
        dcat:Resource ;
    rdfs:label "Item I1131"@en-AU ;
    rdfs:comment "219 U  Renewal of order for detention - GraphNodeID: I1131"@en-AU ;
    skos:definition "219 U  Renewal of order for detention"@en-AU ;
    skos:narrower C1901A00006:1125 ;
    skos:prefLabel "Item I1131"@en-AU ;
    dcat:accessURL "https://www.legislation.gov.au/C1901A00006/2024-07-01/2024-07-01/text/original/epub/OEBPS/document_3/document_3.html#_Toc172627165"^^xsd:anyURI .

C1901A00006:1132 a legcons:Item,
        skos:Concept,
        dcat:Resource ;
    rdfs:label "Item I1132"@en-AU ;
    rdfs:comment "219 V  Arrangement for internal medical search - GraphNodeID: I1132"@en-AU ;
    skos:definition "219 V  Arrangement for internal medical search"@en-AU ;
    skos:narrower C1901A00006:1125 ;
    skos:prefLabel "Item I1132"@en-AU ;
    dcat:accessURL "https://www.legislation.gov.au/C1901A00006/2024-07-01/2024-07-01/text/original/epub/OEBPS/document_3/document_3.html#_Toc172627166"^^xsd:anyURI .

C1901A00006:1133 a legcons:Item,
        skos:Concept,
        dcat:Resource ;
    rdfs:label "Item I1133"@en-AU ;
    rdfs:comment "219 W  Detention under this Subdivision - GraphNodeID: I1133"@en-AU ;
    skos:definition "219 W  Detention under this Subdivision"@en-AU ;
    skos:narrower C1901A00006:1125 ;
    skos:prefLabel "Item I1133"@en-AU ;
    dcat:accessURL "https://www.legislation.gov.au/C1901A00006/2024-07-01/2024-07-01/text/original/epub/OEBPS/document_3/document_3.html#_Toc172627167"^^xsd:anyURI .

C1901A00006:1134 a legcons:Item,
        skos:Concept,
        dcat:Resource ;
    rdfs:label "Item I1134"@en-AU ;
    rdfs:comment "219 X  Detainee becoming in need of protection - GraphNodeID: I1134"@en-AU ;
    skos:definition "219 X  Detainee becoming in need of protection"@en-AU ;
    skos:narrower C1901A00006:1125 ;
    skos:prefLabel "Item I1134"@en-AU ;
    dcat:accessURL "https://www.legislation.gov.au/C1901A00006/2024-07-01/2024-07-01/text/original/epub/OEBPS/document_3/document_3.html#_Toc172627168"^^xsd:anyURI .

C1901A00006:1135 a legcons:Item,
        skos:Concept,
        dcat:Resource ;
    rdfs:label "Item I1135"@en-AU ;
    rdfs:comment "219 Y  Applications for orders under this Subdivision - GraphNodeID: I1135"@en-AU ;
    skos:definition "219 Y  Applications for orders under this Subdivision"@en-AU ;
    skos:narrower C1901A00006:1125 ;
    skos:prefLabel "Item I1135"@en-AU ;
    dcat:accessURL "https://www.legislation.gov.au/C1901A00006/2024-07-01/2024-07-01/text/original/epub/OEBPS/document_3/document_3.html#_Toc172627169"^^xsd:anyURI .

C1901A00006:1136 a legcons:Item,
        skos:Concept,
        dcat:Resource ;
    rdfs:label "Item I1136"@en-AU ;
    rdfs:comment "219 Z  Internal medical search by medical practitioner - GraphNodeID: I1136"@en-AU ;
    skos:definition "219 Z  Internal medical search by medical practitioner"@en-AU ;
    skos:narrower C1901A00006:1125 ;
    skos:prefLabel "Item I1136"@en-AU ;
    dcat:accessURL "https://www.legislation.gov.au/C1901A00006/2024-07-01/2024-07-01/text/original/epub/OEBPS/document_3/document_3.html#_Toc172627170"^^xsd:anyURI .

C1901A00006:1138 a legcons:Item,
        skos:Concept,
        dcat:Resource ;
    rdfs:label "Item I1138"@en-AU ;
    rdfs:comment "219 ZAA  Use of prescribed equipment for external search or internal non medical scan - GraphNodeID: I1138"@en-AU ;
    skos:definition "219 ZAA  Use of prescribed equipment for external search or internal non medical scan"@en-AU ;
    skos:narrower C1901A00006:1137 ;
    skos:prefLabel "Item I1138"@en-AU ;
    dcat:accessURL "https://www.legislation.gov.au/C1901A00006/2024-07-01/2024-07-01/text/original/epub/OEBPS/document_3/document_3.html#_Toc172627172"^^xsd:anyURI .

C1901A00006:1139 a legcons:Item,
        skos:Concept,
        dcat:Resource ;
    rdfs:label "Item I1139"@en-AU ;
    rdfs:comment "219 ZAB  Prescribing equipment for use in external searches and internal non medical scans - GraphNodeID: I1139"@en-AU ;
    skos:definition "219 ZAB  Prescribing equipment for use in external searches and internal non medical scans"@en-AU ;
    skos:narrower C1901A00006:1137 ;
    skos:prefLabel "Item I1139"@en-AU ;
    dcat:accessURL "https://www.legislation.gov.au/C1901A00006/2024-07-01/2024-07-01/text/original/epub/OEBPS/document_3/document_3.html#_Toc172627173"^^xsd:anyURI .

C1901A00006:114 a legcons:Item,
        skos:Concept,
        dcat:Resource ;
    rdfs:label "Item I114"@en-AU ;
    rdfs:comment "67 F  Applying to be a re mail reporter - GraphNodeID: I114"@en-AU ;
    skos:definition "67 F  Applying to be a re mail reporter"@en-AU ;
    skos:narrower C1901A00006:113 ;
    skos:prefLabel "Item I114"@en-AU ;
    dcat:accessURL "https://www.legislation.gov.au/C1901A00006/2024-07-01/2024-07-01/text/original/epub/OEBPS/document_1/document_1.html#_Toc172623088"^^xsd:anyURI .

C1901A00006:1140 a legcons:Item,
        skos:Concept,
        dcat:Resource ;
    rdfs:label "Item I1140"@en-AU ;
    rdfs:comment "219 ZAC  Authorising officers to use prescribed equipment for external search or internal non medical scan - GraphNodeID: I1140"@en-AU ;
    skos:definition "219 ZAC  Authorising officers to use prescribed equipment for external search or internal non medical scan"@en-AU ;
    skos:narrower C1901A00006:1137 ;
    skos:prefLabel "Item I1140"@en-AU ;
    dcat:accessURL "https://www.legislation.gov.au/C1901A00006/2024-07-01/2024-07-01/text/original/epub/OEBPS/document_3/document_3.html#_Toc172627174"^^xsd:anyURI .

C1901A00006:1141 a legcons:Item,
        skos:Concept,
        dcat:Resource ;
    rdfs:label "Item I1141"@en-AU ;
    rdfs:comment "219 ZAD  Giving a record of invitation and consent or a copy of order - GraphNodeID: I1141"@en-AU ;
    skos:definition "219 ZAD  Giving a record of invitation and consent or a copy of order"@en-AU ;
    skos:narrower C1901A00006:1137 ;
    skos:prefLabel "Item I1141"@en-AU ;
    dcat:accessURL "https://www.legislation.gov.au/C1901A00006/2024-07-01/2024-07-01/text/original/epub/OEBPS/document_3/document_3.html#_Toc172627175"^^xsd:anyURI .

C1901A00006:1142 a legcons:Item,
        skos:Concept,
        dcat:Resource ;
    rdfs:label "Item I1142"@en-AU ;
    rdfs:comment "219 ZAE  Records of results of external search or internal non medical scan - GraphNodeID: I1142"@en-AU ;
    skos:definition "219 ZAE  Records of results of external search or internal non medical scan"@en-AU ;
    skos:narrower C1901A00006:1137 ;
    skos:prefLabel "Item I1142"@en-AU ;
    dcat:accessURL "https://www.legislation.gov.au/C1901A00006/2024-07-01/2024-07-01/text/original/epub/OEBPS/document_3/document_3.html#_Toc172627176"^^xsd:anyURI .

C1901A00006:1144 a legcons:Item,
        skos:Concept,
        dcat:Resource ;
    rdfs:label "Item I1144"@en-AU ;
    rdfs:comment "219 ZA  Detention officers - GraphNodeID: I1144"@en-AU ;
    skos:definition "219 ZA  Detention officers"@en-AU ;
    skos:narrower C1901A00006:1143 ;
    skos:prefLabel "Item I1144"@en-AU ;
    dcat:accessURL "https://www.legislation.gov.au/C1901A00006/2024-07-01/2024-07-01/text/original/epub/OEBPS/document_3/document_3.html#_Toc172627178"^^xsd:anyURI .

C1901A00006:1145 a legcons:Item,
        skos:Concept,
        dcat:Resource ;
    rdfs:label "Item I1145"@en-AU ;
    rdfs:comment "219 ZB  Detention places - GraphNodeID: I1145"@en-AU ;
    skos:definition "219 ZB  Detention places"@en-AU ;
    skos:narrower C1901A00006:1143 ;
    skos:prefLabel "Item I1145"@en-AU ;
    dcat:accessURL "https://www.legislation.gov.au/C1901A00006/2024-07-01/2024-07-01/text/original/epub/OEBPS/document_3/document_3.html#_Toc172627179"^^xsd:anyURI .

C1901A00006:1146 a legcons:Item,
        skos:Concept,
        dcat:Resource ;
    rdfs:label "Item I1146"@en-AU ;
    rdfs:comment "219 ZC  Detention under this Division - GraphNodeID: I1146"@en-AU ;
    skos:definition "219 ZC  Detention under this Division"@en-AU ;
    skos:narrower C1901A00006:1143 ;
    skos:prefLabel "Item I1146"@en-AU ;
    dcat:accessURL "https://www.legislation.gov.au/C1901A00006/2024-07-01/2024-07-01/text/original/epub/OEBPS/document_3/document_3.html#_Toc172627180"^^xsd:anyURI .

C1901A00006:1147 a legcons:Item,
        skos:Concept,
        dcat:Resource ;
    rdfs:label "Item I1147"@en-AU ;
    rdfs:comment "219 ZD  Detainees not fluent in English - GraphNodeID: I1147"@en-AU ;
    skos:definition "219 ZD  Detainees not fluent in English"@en-AU ;
    skos:narrower C1901A00006:1143 ;
    skos:prefLabel "Item I1147"@en-AU ;
    dcat:accessURL "https://www.legislation.gov.au/C1901A00006/2024-07-01/2024-07-01/text/original/epub/OEBPS/document_3/document_3.html#_Toc172627181"^^xsd:anyURI .

C1901A00006:1148 a legcons:Item,
        skos:Concept,
        dcat:Resource ;
    rdfs:label "Item I1148"@en-AU ;
    rdfs:comment "219 ZE  Release from or cessation of detention - GraphNodeID: I1148"@en-AU ;
    skos:definition "219 ZE  Release from or cessation of detention"@en-AU ;
    skos:narrower C1901A00006:1143 ;
    skos:prefLabel "Item I1148"@en-AU ;
    dcat:accessURL "https://www.legislation.gov.au/C1901A00006/2024-07-01/2024-07-01/text/original/epub/OEBPS/document_3/document_3.html#_Toc172627182"^^xsd:anyURI .

C1901A00006:115 a legcons:Item,
        skos:Concept,
        dcat:Resource ;
    rdfs:label "Item I115"@en-AU ;
    rdfs:comment "67 G  Registering re mail reporters - GraphNodeID: I115"@en-AU ;
    skos:definition "67 G  Registering re mail reporters"@en-AU ;
    skos:narrower C1901A00006:113 ;
    skos:prefLabel "Item I115"@en-AU ;
    dcat:accessURL "https://www.legislation.gov.au/C1901A00006/2024-07-01/2024-07-01/text/original/epub/OEBPS/document_1/document_1.html#_Toc172623089"^^xsd:anyURI .

C1901A00006:1150 a legcons:Item,
        skos:Concept,
        dcat:Resource ;
    rdfs:label "Item I1150"@en-AU ;
    rdfs:comment "219 ZF  Conduct of internal medical search - GraphNodeID: I1150"@en-AU ;
    skos:definition "219 ZF  Conduct of internal medical search"@en-AU ;
    skos:narrower C1901A00006:1149 ;
    skos:prefLabel "Item I1150"@en-AU ;
    dcat:accessURL "https://www.legislation.gov.au/C1901A00006/2024-07-01/2024-07-01/text/original/epub/OEBPS/document_3/document_3.html#_Toc172627184"^^xsd:anyURI .

C1901A00006:1151 a legcons:Item,
        skos:Concept,
        dcat:Resource ;
    rdfs:label "Item I1151"@en-AU ;
    rdfs:comment "219 ZG  Medical practitioner may take action to preserve detainees life - GraphNodeID: I1151"@en-AU ;
    skos:definition "219 ZG  Medical practitioner may take action to preserve detainees life"@en-AU ;
    skos:narrower C1901A00006:1149 ;
    skos:prefLabel "Item I1151"@en-AU ;
    dcat:accessURL "https://www.legislation.gov.au/C1901A00006/2024-07-01/2024-07-01/text/original/epub/OEBPS/document_3/document_3.html#_Toc172627185"^^xsd:anyURI .

C1901A00006:1152 a legcons:Item,
        skos:Concept,
        dcat:Resource ;
    rdfs:label "Item I1152"@en-AU ;
    rdfs:comment "219 ZH  Medical practitioner to answer questions and prepare report - GraphNodeID: I1152"@en-AU ;
    skos:definition "219 ZH  Medical practitioner to answer questions and prepare report"@en-AU ;
    skos:narrower C1901A00006:1149 ;
    skos:prefLabel "Item I1152"@en-AU ;
    dcat:accessURL "https://www.legislation.gov.au/C1901A00006/2024-07-01/2024-07-01/text/original/epub/OEBPS/document_3/document_3.html#_Toc172627186"^^xsd:anyURI .

C1901A00006:1153 a legcons:Item,
        skos:Concept,
        dcat:Resource ;
    rdfs:label "Item I1153"@en-AU ;
    rdfs:comment "219 ZJ  Proceedings against medical practitioners - GraphNodeID: I1153"@en-AU ;
    skos:definition "219 ZJ  Proceedings against medical practitioners"@en-AU ;
    skos:narrower C1901A00006:1149 ;
    skos:prefLabel "Item I1153"@en-AU ;
    dcat:accessURL "https://www.legislation.gov.au/C1901A00006/2024-07-01/2024-07-01/text/original/epub/OEBPS/document_3/document_3.html#_Toc172627187"^^xsd:anyURI .

C1901A00006:1156 a legcons:Item,
        skos:Concept,
        dcat:Resource ;
    rdfs:label "Item I1156"@en-AU ;
    rdfs:comment "219 ZJA  Definitions - GraphNodeID: I1156"@en-AU ;
    skos:definition "219 ZJA  Definitions"@en-AU ;
    skos:narrower C1901A00006:1155 ;
    skos:prefLabel "Item I1156"@en-AU ;
    dcat:accessURL "https://www.legislation.gov.au/C1901A00006/2024-07-01/2024-07-01/text/original/epub/OEBPS/document_3/document_3.html#_Toc172627190"^^xsd:anyURI .

C1901A00006:1157 a legcons:Item,
        skos:Concept,
        dcat:Resource ;
    rdfs:label "Item I1157"@en-AU ;
    rdfs:comment "219 ZJAA  Prescribed State or Territory offences - GraphNodeID: I1157"@en-AU ;
    skos:definition "219 ZJAA  Prescribed State or Territory offences"@en-AU ;
    skos:narrower C1901A00006:1155 ;
    skos:prefLabel "Item I1157"@en-AU ;
    dcat:accessURL "https://www.legislation.gov.au/C1901A00006/2024-07-01/2024-07-01/text/original/epub/OEBPS/document_3/document_3.html#_Toc172627191"^^xsd:anyURI .

C1901A00006:1159 a legcons:Item,
        skos:Concept,
        dcat:Resource ;
    rdfs:label "Item I1159"@en-AU ;
    rdfs:comment "219 ZJB  Detention of person suspected of committing serious Commonwealth offence or prescribed State or Territory offence - GraphNodeID: I1159"@en-AU ;
    skos:definition "219 ZJB  Detention of person suspected of committing serious Commonwealth offence or prescribed State or Territory offence"@en-AU ;
    skos:narrower C1901A00006:1158 ;
    skos:prefLabel "Item I1159"@en-AU ;
    dcat:accessURL "https://www.legislation.gov.au/C1901A00006/2024-07-01/2024-07-01/text/original/epub/OEBPS/document_3/document_3.html#_Toc172627193"^^xsd:anyURI .

C1901A00006:116 a legcons:Item,
        skos:Concept,
        dcat:Resource ;
    rdfs:label "Item I116"@en-AU ;
    rdfs:comment "67 H  Fit and proper person test - GraphNodeID: I116"@en-AU ;
    skos:definition "67 H  Fit and proper person test"@en-AU ;
    skos:narrower C1901A00006:113 ;
    skos:prefLabel "Item I116"@en-AU ;
    dcat:accessURL "https://www.legislation.gov.au/C1901A00006/2024-07-01/2024-07-01/text/original/epub/OEBPS/document_1/document_1.html#_Toc172623090"^^xsd:anyURI .

C1901A00006:1160 a legcons:Item,
        skos:Concept,
        dcat:Resource ;
    rdfs:label "Item I1160"@en-AU ;
    rdfs:comment "219 ZJC  Detention of person subject to warrant or bail condition - GraphNodeID: I1160"@en-AU ;
    skos:definition "219 ZJC  Detention of person subject to warrant or bail condition"@en-AU ;
    skos:narrower C1901A00006:1158 ;
    skos:prefLabel "Item I1160"@en-AU ;
    dcat:accessURL "https://www.legislation.gov.au/C1901A00006/2024-07-01/2024-07-01/text/original/epub/OEBPS/document_3/document_3.html#_Toc172627194"^^xsd:anyURI .

C1901A00006:1161 a legcons:Item,
        skos:Concept,
        dcat:Resource ;
    rdfs:label "Item I1161"@en-AU ;
    rdfs:comment "219 ZJCA  Detention of person for national security or security of a foreign country - GraphNodeID: I1161"@en-AU ;
    skos:definition "219 ZJCA  Detention of person for national security or security of a foreign country"@en-AU ;
    skos:narrower C1901A00006:1158 ;
    skos:prefLabel "Item I1161"@en-AU ;
    dcat:accessURL "https://www.legislation.gov.au/C1901A00006/2024-07-01/2024-07-01/text/original/epub/OEBPS/document_3/document_3.html#_Toc172627195"^^xsd:anyURI .

C1901A00006:1163 a legcons:Item,
        skos:Concept,
        dcat:Resource ;
    rdfs:label "Item I1163"@en-AU ;
    rdfs:comment "219 ZJD  Search of person detained under this Division - GraphNodeID: I1163"@en-AU ;
    skos:definition "219 ZJD  Search of person detained under this Division"@en-AU ;
    skos:narrower C1901A00006:1162 ;
    skos:prefLabel "Item I1163"@en-AU ;
    dcat:accessURL "https://www.legislation.gov.au/C1901A00006/2024-07-01/2024-07-01/text/original/epub/OEBPS/document_3/document_3.html#_Toc172627197"^^xsd:anyURI .

C1901A00006:1164 a legcons:Item,
        skos:Concept,
        dcat:Resource ;
    rdfs:label "Item I1164"@en-AU ;
    rdfs:comment "219 ZJE  Comptroller General of Customs must give directions about detaining persons under this Division - GraphNodeID: I1164"@en-AU ;
    skos:definition "219 ZJE  Comptroller General of Customs must give directions about detaining persons under this Division"@en-AU ;
    skos:narrower C1901A00006:1162 ;
    skos:prefLabel "Item I1164"@en-AU ;
    dcat:accessURL "https://www.legislation.gov.au/C1901A00006/2024-07-01/2024-07-01/text/original/epub/OEBPS/document_3/document_3.html#_Toc172627198"^^xsd:anyURI .

C1901A00006:1165 a legcons:Item,
        skos:Concept,
        dcat:Resource ;
    rdfs:label "Item I1165"@en-AU ;
    rdfs:comment "219 ZJF  Detainees to be given reasons for detention and shown identification on request - GraphNodeID: I1165"@en-AU ;
    skos:definition "219 ZJF  Detainees to be given reasons for detention and shown identification on request"@en-AU ;
    skos:narrower C1901A00006:1162 ;
    skos:prefLabel "Item I1165"@en-AU ;
    dcat:accessURL "https://www.legislation.gov.au/C1901A00006/2024-07-01/2024-07-01/text/original/epub/OEBPS/document_3/document_3.html#_Toc172627199"^^xsd:anyURI .

C1901A00006:1166 a legcons:Item,
        skos:Concept,
        dcat:Resource ;
    rdfs:label "Item I1166"@en-AU ;
    rdfs:comment "219 ZJG  Use of force in relation to detention - GraphNodeID: I1166"@en-AU ;
    skos:definition "219 ZJG  Use of force in relation to detention"@en-AU ;
    skos:narrower C1901A00006:1162 ;
    skos:prefLabel "Item I1166"@en-AU ;
    dcat:accessURL "https://www.legislation.gov.au/C1901A00006/2024-07-01/2024-07-01/text/original/epub/OEBPS/document_3/document_3.html#_Toc172627200"^^xsd:anyURI .

C1901A00006:1167 a legcons:Item,
        skos:Concept,
        dcat:Resource ;
    rdfs:label "Item I1167"@en-AU ;
    rdfs:comment "219 ZJH  Moving detained persons - GraphNodeID: I1167"@en-AU ;
    skos:definition "219 ZJH  Moving detained persons"@en-AU ;
    skos:narrower C1901A00006:1162 ;
    skos:prefLabel "Item I1167"@en-AU ;
    dcat:accessURL "https://www.legislation.gov.au/C1901A00006/2024-07-01/2024-07-01/text/original/epub/OEBPS/document_3/document_3.html#_Toc172627201"^^xsd:anyURI .

C1901A00006:1168 a legcons:Item,
        skos:Concept,
        dcat:Resource ;
    rdfs:label "Item I1168"@en-AU ;
    rdfs:comment "219 ZJI  Detainees not fluent in English - GraphNodeID: I1168"@en-AU ;
    skos:definition "219 ZJI  Detainees not fluent in English"@en-AU ;
    skos:narrower C1901A00006:1162 ;
    skos:prefLabel "Item I1168"@en-AU ;
    dcat:accessURL "https://www.legislation.gov.au/C1901A00006/2024-07-01/2024-07-01/text/original/epub/OEBPS/document_3/document_3.html#_Toc172627202"^^xsd:anyURI .

C1901A00006:1169 a legcons:Item,
        skos:Concept,
        dcat:Resource ;
    rdfs:label "Item I1169"@en-AU ;
    rdfs:comment "219 ZJJ  Detention of minors - GraphNodeID: I1169"@en-AU ;
    skos:definition "219 ZJJ  Detention of minors"@en-AU ;
    skos:narrower C1901A00006:1162 ;
    skos:prefLabel "Item I1169"@en-AU ;
    dcat:accessURL "https://www.legislation.gov.au/C1901A00006/2024-07-01/2024-07-01/text/original/epub/OEBPS/document_3/document_3.html#_Toc172627203"^^xsd:anyURI .

C1901A00006:117 a legcons:Item,
        skos:Concept,
        dcat:Resource ;
    rdfs:label "Item I117"@en-AU ;
    rdfs:comment "67 I  Obligation of re mail reporters to notify Comptroller General of Customs of certain matters - GraphNodeID: I117"@en-AU ;
    skos:definition "67 I  Obligation of re mail reporters to notify Comptroller General of Customs of certain matters"@en-AU ;
    skos:narrower C1901A00006:113 ;
    skos:prefLabel "Item I117"@en-AU ;
    dcat:accessURL "https://www.legislation.gov.au/C1901A00006/2024-07-01/2024-07-01/text/original/epub/OEBPS/document_1/document_1.html#_Toc172623091"^^xsd:anyURI .

C1901A00006:1170 a legcons:Division,
        skos:Concept,
        dcat:Resource ;
    rdfs:label "Division D1170"@en-AU ;
    rdfs:comment "Division 1 CJudges and Magistrates - GraphNodeID: D1170"@en-AU ;
    skos:definition "Division 1 CJudges and Magistrates"@en-AU ;
    skos:narrower C1901A00006:953 ;
    skos:prefLabel "Division D1170"@en-AU ;
    dcat:accessURL "https://www.legislation.gov.au/C1901A00006/2024-07-01/2024-07-01/text/original/epub/OEBPS/document_3/document_3.html#_Toc172627204"^^xsd:anyURI .

C1901A00006:1171 a legcons:Item,
        skos:Concept,
        dcat:Resource ;
    rdfs:label "Item I1171"@en-AU ;
    rdfs:comment "219 ZK  Nature of functions of Judge or Magistrate - GraphNodeID: I1171"@en-AU ;
    skos:definition "219 ZK  Nature of functions of Judge or Magistrate"@en-AU ;
    skos:narrower C1901A00006:1162 ;
    skos:prefLabel "Item I1171"@en-AU ;
    dcat:accessURL "https://www.legislation.gov.au/C1901A00006/2024-07-01/2024-07-01/text/original/epub/OEBPS/document_3/document_3.html#_Toc172627205"^^xsd:anyURI .

C1901A00006:1172 a legcons:Item,
        skos:Concept,
        dcat:Resource ;
    rdfs:label "Item I1172"@en-AU ;
    rdfs:comment "219 ZL  Protection of Judge or Magistrate - GraphNodeID: I1172"@en-AU ;
    skos:definition "219 ZL  Protection of Judge or Magistrate"@en-AU ;
    skos:narrower C1901A00006:1162 ;
    skos:prefLabel "Item I1172"@en-AU ;
    dcat:accessURL "https://www.legislation.gov.au/C1901A00006/2024-07-01/2024-07-01/text/original/epub/OEBPS/document_3/document_3.html#_Toc172627206"^^xsd:anyURI .

C1901A00006:1173 a legcons:Division,
        skos:Concept,
        dcat:Resource ;
    rdfs:label "Division D1173"@en-AU ;
    rdfs:comment "Division 2 Protection to officers - GraphNodeID: D1173"@en-AU ;
    skos:definition "Division 2 Protection to officers"@en-AU ;
    skos:narrower C1901A00006:953 ;
    skos:prefLabel "Division D1173"@en-AU ;
    dcat:accessURL "https://www.legislation.gov.au/C1901A00006/2024-07-01/2024-07-01/text/original/epub/OEBPS/document_3/document_3.html#_Toc172627207"^^xsd:anyURI .

C1901A00006:1174 a legcons:Item,
        skos:Concept,
        dcat:Resource ;
    rdfs:label "Item I1174"@en-AU ;
    rdfs:comment "220  Reasonable cause for seizure a bar to action - GraphNodeID: I1174"@en-AU ;
    skos:definition "220  Reasonable cause for seizure a bar to action"@en-AU ;
    skos:narrower C1901A00006:1162 ;
    skos:prefLabel "Item I1174"@en-AU ;
    dcat:accessURL "https://www.legislation.gov.au/C1901A00006/2024-07-01/2024-07-01/text/original/epub/OEBPS/document_3/document_3.html#_Toc172627208"^^xsd:anyURI .

C1901A00006:1175 a legcons:Item,
        skos:Concept,
        dcat:Resource ;
    rdfs:label "Item I1175"@en-AU ;
    rdfs:comment "221  Notice of action to be given - GraphNodeID: I1175"@en-AU ;
    skos:definition "221  Notice of action to be given"@en-AU ;
    skos:narrower C1901A00006:1162 ;
    skos:prefLabel "Item I1175"@en-AU ;
    dcat:accessURL "https://www.legislation.gov.au/C1901A00006/2024-07-01/2024-07-01/text/original/epub/OEBPS/document_3/document_3.html#_Toc172627209"^^xsd:anyURI .

C1901A00006:1176 a legcons:Item,
        skos:Concept,
        dcat:Resource ;
    rdfs:label "Item I1176"@en-AU ;
    rdfs:comment "222  Defect in notice not to invalidate - GraphNodeID: I1176"@en-AU ;
    skos:definition "222  Defect in notice not to invalidate"@en-AU ;
    skos:narrower C1901A00006:1162 ;
    skos:prefLabel "Item I1176"@en-AU ;
    dcat:accessURL "https://www.legislation.gov.au/C1901A00006/2024-07-01/2024-07-01/text/original/epub/OEBPS/document_3/document_3.html#_Toc172627210"^^xsd:anyURI .

C1901A00006:1177 a legcons:Item,
        skos:Concept,
        dcat:Resource ;
    rdfs:label "Item I1177"@en-AU ;
    rdfs:comment "223  No evidence to be produced but that contained in notice - GraphNodeID: I1177"@en-AU ;
    skos:definition "223  No evidence to be produced but that contained in notice"@en-AU ;
    skos:narrower C1901A00006:1162 ;
    skos:prefLabel "Item I1177"@en-AU ;
    dcat:accessURL "https://www.legislation.gov.au/C1901A00006/2024-07-01/2024-07-01/text/original/epub/OEBPS/document_3/document_3.html#_Toc172627211"^^xsd:anyURI .

C1901A00006:1178 a legcons:Item,
        skos:Concept,
        dcat:Resource ;
    rdfs:label "Item I1178"@en-AU ;
    rdfs:comment "224  Officer may tender amends - GraphNodeID: I1178"@en-AU ;
    skos:definition "224  Officer may tender amends"@en-AU ;
    skos:narrower C1901A00006:1162 ;
    skos:prefLabel "Item I1178"@en-AU ;
    dcat:accessURL "https://www.legislation.gov.au/C1901A00006/2024-07-01/2024-07-01/text/original/epub/OEBPS/document_3/document_3.html#_Toc172627212"^^xsd:anyURI .

C1901A00006:1179 a legcons:Item,
        skos:Concept,
        dcat:Resource ;
    rdfs:label "Item I1179"@en-AU ;
    rdfs:comment "225  Commencement of proceedings against officers - GraphNodeID: I1179"@en-AU ;
    skos:definition "225  Commencement of proceedings against officers"@en-AU ;
    skos:narrower C1901A00006:1162 ;
    skos:prefLabel "Item I1179"@en-AU ;
    dcat:accessURL "https://www.legislation.gov.au/C1901A00006/2024-07-01/2024-07-01/text/original/epub/OEBPS/document_3/document_3.html#_Toc172627213"^^xsd:anyURI .

C1901A00006:118 a legcons:Item,
        skos:Concept,
        dcat:Resource ;
    rdfs:label "Item I118"@en-AU ;
    rdfs:comment "67 J  Varying etc conditions of registration - GraphNodeID: I118"@en-AU ;
    skos:definition "67 J  Varying etc conditions of registration"@en-AU ;
    skos:narrower C1901A00006:113 ;
    skos:prefLabel "Item I118"@en-AU ;
    dcat:accessURL "https://www.legislation.gov.au/C1901A00006/2024-07-01/2024-07-01/text/original/epub/OEBPS/document_1/document_1.html#_Toc172623092"^^xsd:anyURI .

C1901A00006:1180 a legcons:Item,
        skos:Concept,
        dcat:Resource ;
    rdfs:label "Item I1180"@en-AU ;
    rdfs:comment "226  Time for commencing action - GraphNodeID: I1180"@en-AU ;
    skos:definition "226  Time for commencing action"@en-AU ;
    skos:narrower C1901A00006:1162 ;
    skos:prefLabel "Item I1180"@en-AU ;
    dcat:accessURL "https://www.legislation.gov.au/C1901A00006/2024-07-01/2024-07-01/text/original/epub/OEBPS/document_3/document_3.html#_Toc172627214"^^xsd:anyURI .

C1901A00006:1181 a legcons:Item,
        skos:Concept,
        dcat:Resource ;
    rdfs:label "Item I1181"@en-AU ;
    rdfs:comment "227  Security may be required - GraphNodeID: I1181"@en-AU ;
    skos:definition "227  Security may be required"@en-AU ;
    skos:narrower C1901A00006:1162 ;
    skos:prefLabel "Item I1181"@en-AU ;
    dcat:accessURL "https://www.legislation.gov.au/C1901A00006/2024-07-01/2024-07-01/text/original/epub/OEBPS/document_3/document_3.html#_Toc172627215"^^xsd:anyURI .

C1901A00006:1182 a legcons:Division,
        skos:Concept,
        dcat:Resource ;
    rdfs:label "Division D1182"@en-AU ;
    rdfs:comment "Division 3 Evidence - GraphNodeID: D1182"@en-AU ;
    skos:definition "Division 3 Evidence"@en-AU ;
    skos:narrower C1901A00006:953 ;
    skos:prefLabel "Division D1182"@en-AU ;
    dcat:accessURL "https://www.legislation.gov.au/C1901A00006/2024-07-01/2024-07-01/text/original/epub/OEBPS/document_3/document_3.html#_Toc172627216"^^xsd:anyURI .

C1901A00006:1183 a legcons:Item,
        skos:Concept,
        dcat:Resource ;
    rdfs:label "Item I1183"@en-AU ;
    rdfs:comment "227 AA  Evidence may be used in prosecutions etc - GraphNodeID: I1183"@en-AU ;
    skos:definition "227 AA  Evidence may be used in prosecutions etc"@en-AU ;
    skos:narrower C1901A00006:1162 ;
    skos:prefLabel "Item I1183"@en-AU ;
    dcat:accessURL "https://www.legislation.gov.au/C1901A00006/2024-07-01/2024-07-01/text/original/epub/OEBPS/document_3/document_3.html#_Toc172627217"^^xsd:anyURI .

C1901A00006:1184 a legcons:Part,
        skos:Concept,
        dcat:Resource ;
    rdfs:label "Part P1184"@en-AU ;
    rdfs:comment "Part XIIASpecial provisions relating to prohibited items - GraphNodeID: P1184"@en-AU ;
    skos:definition "Part XIIASpecial provisions relating to prohibited items"@en-AU ;
    skos:narrower C1901A00006:952 ;
    skos:prefLabel "Part P1184"@en-AU ;
    dcat:accessURL "https://www.legislation.gov.au/C1901A00006/2024-07-01/2024-07-01/text/original/epub/OEBPS/document_3/document_3.html#_Toc172627218"^^xsd:anyURI .

C1901A00006:1185 a legcons:Item,
        skos:Concept,
        dcat:Resource ;
    rdfs:label "Item I1185"@en-AU ;
    rdfs:comment "227 A  Overview of Part - GraphNodeID: I1185"@en-AU ;
    skos:definition "227 A  Overview of Part"@en-AU ;
    skos:narrower C1901A00006:1162 ;
    skos:prefLabel "Item I1185"@en-AU ;
    dcat:accessURL "https://www.legislation.gov.au/C1901A00006/2024-07-01/2024-07-01/text/original/epub/OEBPS/document_3/document_3.html#_Toc172627219"^^xsd:anyURI .

C1901A00006:1186 a legcons:Item,
        skos:Concept,
        dcat:Resource ;
    rdfs:label "Item I1186"@en-AU ;
    rdfs:comment "227 B  Definitions - GraphNodeID: I1186"@en-AU ;
    skos:definition "227 B  Definitions"@en-AU ;
    skos:narrower C1901A00006:1162 ;
    skos:prefLabel "Item I1186"@en-AU ;
    dcat:accessURL "https://www.legislation.gov.au/C1901A00006/2024-07-01/2024-07-01/text/original/epub/OEBPS/document_3/document_3.html#_Toc172627220"^^xsd:anyURI .

C1901A00006:1187 a legcons:Item,
        skos:Concept,
        dcat:Resource ;
    rdfs:label "Item I1187"@en-AU ;
    rdfs:comment "227 C  Ships and aircraft to which this Part applies - GraphNodeID: I1187"@en-AU ;
    skos:definition "227 C  Ships and aircraft to which this Part applies"@en-AU ;
    skos:narrower C1901A00006:1162 ;
    skos:prefLabel "Item I1187"@en-AU ;
    dcat:accessURL "https://www.legislation.gov.au/C1901A00006/2024-07-01/2024-07-01/text/original/epub/OEBPS/document_3/document_3.html#_Toc172627221"^^xsd:anyURI .

C1901A00006:1188 a legcons:Item,
        skos:Concept,
        dcat:Resource ;
    rdfs:label "Item I1188"@en-AU ;
    rdfs:comment "227 D  Items to which this Part applies - GraphNodeID: I1188"@en-AU ;
    skos:definition "227 D  Items to which this Part applies"@en-AU ;
    skos:narrower C1901A00006:1162 ;
    skos:prefLabel "Item I1188"@en-AU ;
    dcat:accessURL "https://www.legislation.gov.au/C1901A00006/2024-07-01/2024-07-01/text/original/epub/OEBPS/document_3/document_3.html#_Toc172627222"^^xsd:anyURI .

C1901A00006:1189 a legcons:Item,
        skos:Concept,
        dcat:Resource ;
    rdfs:label "Item I1189"@en-AU ;
    rdfs:comment "227 E  Approved storage for prohibited items - GraphNodeID: I1189"@en-AU ;
    skos:definition "227 E  Approved storage for prohibited items"@en-AU ;
    skos:narrower C1901A00006:1162 ;
    skos:prefLabel "Item I1189"@en-AU ;
    dcat:accessURL "https://www.legislation.gov.au/C1901A00006/2024-07-01/2024-07-01/text/original/epub/OEBPS/document_3/document_3.html#_Toc172627223"^^xsd:anyURI .

C1901A00006:119 a legcons:Item,
        skos:Concept,
        dcat:Resource ;
    rdfs:label "Item I119"@en-AU ;
    rdfs:comment "67 K  Cancelling the registration of a re mail reporter - GraphNodeID: I119"@en-AU ;
    skos:definition "67 K  Cancelling the registration of a re mail reporter"@en-AU ;
    skos:narrower C1901A00006:113 ;
    skos:prefLabel "Item I119"@en-AU ;
    dcat:accessURL "https://www.legislation.gov.au/C1901A00006/2024-07-01/2024-07-01/text/original/epub/OEBPS/document_1/document_1.html#_Toc172623093"^^xsd:anyURI .

C1901A00006:1190 a legcons:Item,
        skos:Concept,
        dcat:Resource ;
    rdfs:label "Item I1190"@en-AU ;
    rdfs:comment "227 F  Officer may take custody of items - GraphNodeID: I1190"@en-AU ;
    skos:definition "227 F  Officer may take custody of items"@en-AU ;
    skos:narrower C1901A00006:1162 ;
    skos:prefLabel "Item I1190"@en-AU ;
    dcat:accessURL "https://www.legislation.gov.au/C1901A00006/2024-07-01/2024-07-01/text/original/epub/OEBPS/document_3/document_3.html#_Toc172627224"^^xsd:anyURI .

C1901A00006:1191 a legcons:Item,
        skos:Concept,
        dcat:Resource ;
    rdfs:label "Item I1191"@en-AU ;
    rdfs:comment "227 G  Compensation for damage etc to items - GraphNodeID: I1191"@en-AU ;
    skos:definition "227 G  Compensation for damage etc to items"@en-AU ;
    skos:narrower C1901A00006:1162 ;
    skos:prefLabel "Item I1191"@en-AU ;
    dcat:accessURL "https://www.legislation.gov.au/C1901A00006/2024-07-01/2024-07-01/text/original/epub/OEBPS/document_3/document_3.html#_Toc172627225"^^xsd:anyURI .

C1901A00006:1193 a legcons:Division,
        skos:Concept,
        dcat:Resource ;
    rdfs:label "Division D1193"@en-AU ;
    rdfs:comment "Division 1 Forfeitures - GraphNodeID: D1193"@en-AU ;
    skos:definition "Division 1 Forfeitures"@en-AU ;
    skos:narrower C1901A00006:1192 ;
    skos:prefLabel "Division D1193"@en-AU ;
    dcat:accessURL "https://www.legislation.gov.au/C1901A00006/2024-07-01/2024-07-01/text/original/epub/OEBPS/document_3/document_3.html#_Toc172627227"^^xsd:anyURI .

C1901A00006:1194 a legcons:Item,
        skos:Concept,
        dcat:Resource ;
    rdfs:label "Item I1194"@en-AU ;
    rdfs:comment "228  Forfeited ships and aircraft - GraphNodeID: I1194"@en-AU ;
    skos:definition "228  Forfeited ships and aircraft"@en-AU ;
    skos:narrower C1901A00006:1162 ;
    skos:prefLabel "Item I1194"@en-AU ;
    dcat:accessURL "https://www.legislation.gov.au/C1901A00006/2024-07-01/2024-07-01/text/original/epub/OEBPS/document_3/document_3.html#_Toc172627228"^^xsd:anyURI .

C1901A00006:1195 a legcons:Item,
        skos:Concept,
        dcat:Resource ;
    rdfs:label "Item I1195"@en-AU ;
    rdfs:comment "228 A  Forfeited resources installations - GraphNodeID: I1195"@en-AU ;
    skos:definition "228 A  Forfeited resources installations"@en-AU ;
    skos:narrower C1901A00006:1162 ;
    skos:prefLabel "Item I1195"@en-AU ;
    dcat:accessURL "https://www.legislation.gov.au/C1901A00006/2024-07-01/2024-07-01/text/original/epub/OEBPS/document_3/document_3.html#_Toc172627229"^^xsd:anyURI .

C1901A00006:1196 a legcons:Item,
        skos:Concept,
        dcat:Resource ;
    rdfs:label "Item I1196"@en-AU ;
    rdfs:comment "228 B  Forfeited sea installations - GraphNodeID: I1196"@en-AU ;
    skos:definition "228 B  Forfeited sea installations"@en-AU ;
    skos:narrower C1901A00006:1162 ;
    skos:prefLabel "Item I1196"@en-AU ;
    dcat:accessURL "https://www.legislation.gov.au/C1901A00006/2024-07-01/2024-07-01/text/original/epub/OEBPS/document_3/document_3.html#_Toc172627230"^^xsd:anyURI .

C1901A00006:1197 a legcons:Item,
        skos:Concept,
        dcat:Resource ;
    rdfs:label "Item I1197"@en-AU ;
    rdfs:comment "228 C  Forfeited offshore electricity installations - GraphNodeID: I1197"@en-AU ;
    skos:definition "228 C  Forfeited offshore electricity installations"@en-AU ;
    skos:narrower C1901A00006:1162 ;
    skos:prefLabel "Item I1197"@en-AU ;
    dcat:accessURL "https://www.legislation.gov.au/C1901A00006/2024-07-01/2024-07-01/text/original/epub/OEBPS/document_3/document_3.html#_Toc172627231"^^xsd:anyURI .

C1901A00006:1198 a legcons:Item,
        skos:Concept,
        dcat:Resource ;
    rdfs:label "Item I1198"@en-AU ;
    rdfs:comment "229  Forfeited goods - GraphNodeID: I1198"@en-AU ;
    skos:definition "229  Forfeited goods"@en-AU ;
    skos:narrower C1901A00006:1162 ;
    skos:prefLabel "Item I1198"@en-AU ;
    dcat:accessURL "https://www.legislation.gov.au/C1901A00006/2024-07-01/2024-07-01/text/original/epub/OEBPS/document_3/document_3.html#_Toc172627232"^^xsd:anyURI .

C1901A00006:1199 a legcons:Item,
        skos:Concept,
        dcat:Resource ;
    rdfs:label "Item I1199"@en-AU ;
    rdfs:comment "229 A  Proceeds of drug trafficking liable to forfeiture - GraphNodeID: I1199"@en-AU ;
    skos:definition "229 A  Proceeds of drug trafficking liable to forfeiture"@en-AU ;
    skos:narrower C1901A00006:1162 ;
    skos:prefLabel "Item I1199"@en-AU ;
    dcat:accessURL "https://www.legislation.gov.au/C1901A00006/2024-07-01/2024-07-01/text/original/epub/OEBPS/document_3/document_3.html#_Toc172627233"^^xsd:anyURI .

C1901A00006:12 a legcons:Item,
        skos:Concept,
        dcat:Resource ;
    rdfs:label "Item I12"@en-AU ;
    rdfs:comment "5  Penalties at foot of sections or subsections - GraphNodeID: I12"@en-AU ;
    skos:definition "5  Penalties at foot of sections or subsections"@en-AU ;
    skos:narrower C1901A00006:2 ;
    skos:prefLabel "Item I12"@en-AU ;
    dcat:accessURL "https://www.legislation.gov.au/C1901A00006/2024-07-01/2024-07-01/text/original/epub/OEBPS/document_1/document_1.html#_Toc172622986"^^xsd:anyURI .

C1901A00006:1200 a legcons:Item,
        skos:Concept,
        dcat:Resource ;
    rdfs:label "Item I1200"@en-AU ;
    rdfs:comment "230  Forfeited packages and goods - GraphNodeID: I1200"@en-AU ;
    skos:definition "230  Forfeited packages and goods"@en-AU ;
    skos:narrower C1901A00006:1162 ;
    skos:prefLabel "Item I1200"@en-AU ;
    dcat:accessURL "https://www.legislation.gov.au/C1901A00006/2024-07-01/2024-07-01/text/original/epub/OEBPS/document_3/document_3.html#_Toc172627234"^^xsd:anyURI .

C1901A00006:1201 a legcons:Division,
        skos:Concept,
        dcat:Resource ;
    rdfs:label "Division D1201"@en-AU ;
    rdfs:comment "Division 2 Penalties - GraphNodeID: D1201"@en-AU ;
    skos:definition "Division 2 Penalties"@en-AU ;
    skos:narrower C1901A00006:1192 ;
    skos:prefLabel "Division D1201"@en-AU ;
    dcat:accessURL "https://www.legislation.gov.au/C1901A00006/2024-07-01/2024-07-01/text/original/epub/OEBPS/document_3/document_3.html#_Toc172627235"^^xsd:anyURI .

C1901A00006:1202 a legcons:Item,
        skos:Concept,
        dcat:Resource ;
    rdfs:label "Item I1202"@en-AU ;
    rdfs:comment "231  Assembly for unlawful purposes - GraphNodeID: I1202"@en-AU ;
    skos:definition "231  Assembly for unlawful purposes"@en-AU ;
    skos:narrower C1901A00006:1162 ;
    skos:prefLabel "Item I1202"@en-AU ;
    dcat:accessURL "https://www.legislation.gov.au/C1901A00006/2024-07-01/2024-07-01/text/original/epub/OEBPS/document_3/document_3.html#_Toc172627236"^^xsd:anyURI .

C1901A00006:1203 a legcons:Item,
        skos:Concept,
        dcat:Resource ;
    rdfs:label "Item I1203"@en-AU ;
    rdfs:comment "232 A  Rescuing goods and assaulting officers - GraphNodeID: I1203"@en-AU ;
    skos:definition "232 A  Rescuing goods and assaulting officers"@en-AU ;
    skos:narrower C1901A00006:1162 ;
    skos:prefLabel "Item I1203"@en-AU ;
    dcat:accessURL "https://www.legislation.gov.au/C1901A00006/2024-07-01/2024-07-01/text/original/epub/OEBPS/document_3/document_3.html#_Toc172627237"^^xsd:anyURI .

C1901A00006:1204 a legcons:Item,
        skos:Concept,
        dcat:Resource ;
    rdfs:label "Item I1204"@en-AU ;
    rdfs:comment "233  Smuggling and unlawful importation and exportation - GraphNodeID: I1204"@en-AU ;
    skos:definition "233  Smuggling and unlawful importation and exportation"@en-AU ;
    skos:narrower C1901A00006:1162 ;
    skos:prefLabel "Item I1204"@en-AU ;
    dcat:accessURL "https://www.legislation.gov.au/C1901A00006/2024-07-01/2024-07-01/text/original/epub/OEBPS/document_3/document_3.html#_Toc172627238"^^xsd:anyURI .

C1901A00006:1205 a legcons:Item,
        skos:Concept,
        dcat:Resource ;
    rdfs:label "Item I1205"@en-AU ;
    rdfs:comment "233 A  Master not to use or allow use of ship for smuggling etc - GraphNodeID: I1205"@en-AU ;
    skos:definition "233 A  Master not to use or allow use of ship for smuggling etc"@en-AU ;
    skos:narrower C1901A00006:1162 ;
    skos:prefLabel "Item I1205"@en-AU ;
    dcat:accessURL "https://www.legislation.gov.au/C1901A00006/2024-07-01/2024-07-01/text/original/epub/OEBPS/document_3/document_3.html#_Toc172627239"^^xsd:anyURI .

C1901A00006:1206 a legcons:Item,
        skos:Concept,
        dcat:Resource ;
    rdfs:label "Item I1206"@en-AU ;
    rdfs:comment "233 AB  Penalties for offences against sections 233 and 233 A - GraphNodeID: I1206"@en-AU ;
    skos:definition "233 AB  Penalties for offences against sections 233 and 233 A"@en-AU ;
    skos:narrower C1901A00006:1162 ;
    skos:prefLabel "Item I1206"@en-AU ;
    dcat:accessURL "https://www.legislation.gov.au/C1901A00006/2024-07-01/2024-07-01/text/original/epub/OEBPS/document_3/document_3.html#_Toc172627240"^^xsd:anyURI .

C1901A00006:1207 a legcons:Item,
        skos:Concept,
        dcat:Resource ;
    rdfs:label "Item I1207"@en-AU ;
    rdfs:comment "233 BAA  Special offence relating to tier 1 goods - GraphNodeID: I1207"@en-AU ;
    skos:definition "233 BAA  Special offence relating to tier 1 goods"@en-AU ;
    skos:narrower C1901A00006:1162 ;
    skos:prefLabel "Item I1207"@en-AU ;
    dcat:accessURL "https://www.legislation.gov.au/C1901A00006/2024-07-01/2024-07-01/text/original/epub/OEBPS/document_3/document_3.html#_Toc172627241"^^xsd:anyURI .

C1901A00006:1208 a legcons:Item,
        skos:Concept,
        dcat:Resource ;
    rdfs:label "Item I1208"@en-AU ;
    rdfs:comment "233 BAB  Special offence relating to tier 2 goods - GraphNodeID: I1208"@en-AU ;
    skos:definition "233 BAB  Special offence relating to tier 2 goods"@en-AU ;
    skos:narrower C1901A00006:1162 ;
    skos:prefLabel "Item I1208"@en-AU ;
    dcat:accessURL "https://www.legislation.gov.au/C1901A00006/2024-07-01/2024-07-01/text/original/epub/OEBPS/document_3/document_3.html#_Toc172627242"^^xsd:anyURI .

C1901A00006:1209 a legcons:Item,
        skos:Concept,
        dcat:Resource ;
    rdfs:label "Item I1209"@en-AU ;
    rdfs:comment "233 BABAA  UN sanctioned goods - GraphNodeID: I1209"@en-AU ;
    skos:definition "233 BABAA  UN sanctioned goods"@en-AU ;
    skos:narrower C1901A00006:1162 ;
    skos:prefLabel "Item I1209"@en-AU ;
    dcat:accessURL "https://www.legislation.gov.au/C1901A00006/2024-07-01/2024-07-01/text/original/epub/OEBPS/document_3/document_3.html#_Toc172627243"^^xsd:anyURI .

C1901A00006:1210 a legcons:Item,
        skos:Concept,
        dcat:Resource ;
    rdfs:label "Item I1210"@en-AU ;
    rdfs:comment "233 BABAB  Special offences for importation of UN sanctioned goods - GraphNodeID: I1210"@en-AU ;
    skos:definition "233 BABAB  Special offences for importation of UN sanctioned goods"@en-AU ;
    skos:narrower C1901A00006:1162 ;
    skos:prefLabel "Item I1210"@en-AU ;
    dcat:accessURL "https://www.legislation.gov.au/C1901A00006/2024-07-01/2024-07-01/text/original/epub/OEBPS/document_3/document_3.html#_Toc172627244"^^xsd:anyURI .

C1901A00006:1211 a legcons:Item,
        skos:Concept,
        dcat:Resource ;
    rdfs:label "Item I1211"@en-AU ;
    rdfs:comment "233 BABAC  Special offences for exportation of UN sanctioned goods - GraphNodeID: I1211"@en-AU ;
    skos:definition "233 BABAC  Special offences for exportation of UN sanctioned goods"@en-AU ;
    skos:narrower C1901A00006:1162 ;
    skos:prefLabel "Item I1211"@en-AU ;
    dcat:accessURL "https://www.legislation.gov.au/C1901A00006/2024-07-01/2024-07-01/text/original/epub/OEBPS/document_3/document_3.html#_Toc172627245"^^xsd:anyURI .

C1901A00006:1212 a legcons:Item,
        skos:Concept,
        dcat:Resource ;
    rdfs:label "Item I1212"@en-AU ;
    rdfs:comment "233 BABAD  Offences involving tobacco products - GraphNodeID: I1212"@en-AU ;
    skos:definition "233 BABAD  Offences involving tobacco products"@en-AU ;
    skos:narrower C1901A00006:1162 ;
    skos:prefLabel "Item I1212"@en-AU ;
    dcat:accessURL "https://www.legislation.gov.au/C1901A00006/2024-07-01/2024-07-01/text/original/epub/OEBPS/document_3/document_3.html#_Toc172627246"^^xsd:anyURI .

C1901A00006:1213 a legcons:Item,
        skos:Concept,
        dcat:Resource ;
    rdfs:label "Item I1213"@en-AU ;
    rdfs:comment "233 BABAE  Offence for bringing restricted goods into Australia - GraphNodeID: I1213"@en-AU ;
    skos:definition "233 BABAE  Offence for bringing restricted goods into Australia"@en-AU ;
    skos:narrower C1901A00006:1162 ;
    skos:prefLabel "Item I1213"@en-AU ;
    dcat:accessURL "https://www.legislation.gov.au/C1901A00006/2024-07-01/2024-07-01/text/original/epub/OEBPS/document_3/document_3.html#_Toc172627247"^^xsd:anyURI .

C1901A00006:1214 a legcons:Item,
        skos:Concept,
        dcat:Resource ;
    rdfs:label "Item I1214"@en-AU ;
    rdfs:comment "233 BABAF  Using information held by the Commonwealth - GraphNodeID: I1214"@en-AU ;
    skos:definition "233 BABAF  Using information held by the Commonwealth"@en-AU ;
    skos:narrower C1901A00006:1162 ;
    skos:prefLabel "Item I1214"@en-AU ;
    dcat:accessURL "https://www.legislation.gov.au/C1901A00006/2024-07-01/2024-07-01/text/original/epub/OEBPS/document_3/document_3.html#_Toc172627248"^^xsd:anyURI .

C1901A00006:1215 a legcons:Item,
        skos:Concept,
        dcat:Resource ;
    rdfs:label "Item I1215"@en-AU ;
    rdfs:comment "233 BABA  Protection from criminal responsibility - GraphNodeID: I1215"@en-AU ;
    skos:definition "233 BABA  Protection from criminal responsibility"@en-AU ;
    skos:narrower C1901A00006:1162 ;
    skos:prefLabel "Item I1215"@en-AU ;
    dcat:accessURL "https://www.legislation.gov.au/C1901A00006/2024-07-01/2024-07-01/text/original/epub/OEBPS/document_3/document_3.html#_Toc172627249"^^xsd:anyURI .

C1901A00006:1216 a legcons:Item,
        skos:Concept,
        dcat:Resource ;
    rdfs:label "Item I1216"@en-AU ;
    rdfs:comment "233 BAC  Evidence relating to approval for import or export - GraphNodeID: I1216"@en-AU ;
    skos:definition "233 BAC  Evidence relating to approval for import or export"@en-AU ;
    skos:narrower C1901A00006:1162 ;
    skos:prefLabel "Item I1216"@en-AU ;
    dcat:accessURL "https://www.legislation.gov.au/C1901A00006/2024-07-01/2024-07-01/text/original/epub/OEBPS/document_3/document_3.html#_Toc172627250"^^xsd:anyURI .

C1901A00006:1217 a legcons:Item,
        skos:Concept,
        dcat:Resource ;
    rdfs:label "Item I1217"@en-AU ;
    rdfs:comment "233 BA  Evidence of Analyst - GraphNodeID: I1217"@en-AU ;
    skos:definition "233 BA  Evidence of Analyst"@en-AU ;
    skos:narrower C1901A00006:1162 ;
    skos:prefLabel "Item I1217"@en-AU ;
    dcat:accessURL "https://www.legislation.gov.au/C1901A00006/2024-07-01/2024-07-01/text/original/epub/OEBPS/document_3/document_3.html#_Toc172627251"^^xsd:anyURI .

C1901A00006:1218 a legcons:Item,
        skos:Concept,
        dcat:Resource ;
    rdfs:label "Item I1218"@en-AU ;
    rdfs:comment "233 C  Offence for giving false or misleading information in relation to UN sanctioned goods - GraphNodeID: I1218"@en-AU ;
    skos:definition "233 C  Offence for giving false or misleading information in relation to UN sanctioned goods"@en-AU ;
    skos:narrower C1901A00006:1162 ;
    skos:prefLabel "Item I1218"@en-AU ;
    dcat:accessURL "https://www.legislation.gov.au/C1901A00006/2024-07-01/2024-07-01/text/original/epub/OEBPS/document_3/document_3.html#_Toc172627252"^^xsd:anyURI .

C1901A00006:1219 a legcons:Item,
        skos:Concept,
        dcat:Resource ;
    rdfs:label "Item I1219"@en-AU ;
    rdfs:comment "234  Customs offences - GraphNodeID: I1219"@en-AU ;
    skos:definition "234  Customs offences"@en-AU ;
    skos:narrower C1901A00006:1162 ;
    skos:prefLabel "Item I1219"@en-AU ;
    dcat:accessURL "https://www.legislation.gov.au/C1901A00006/2024-07-01/2024-07-01/text/original/epub/OEBPS/document_3/document_3.html#_Toc172627253"^^xsd:anyURI .

C1901A00006:122 a legcons:Item,
        skos:Concept,
        dcat:Resource ;
    rdfs:label "Item I122"@en-AU ;
    rdfs:comment "68  Entry of imported goods - GraphNodeID: I122"@en-AU ;
    skos:definition "68  Entry of imported goods"@en-AU ;
    skos:narrower C1901A00006:121 ;
    skos:prefLabel "Item I122"@en-AU ;
    dcat:accessURL "https://www.legislation.gov.au/C1901A00006/2024-07-01/2024-07-01/text/original/epub/OEBPS/document_1/document_1.html#_Toc172623096"^^xsd:anyURI .

C1901A00006:1220 a legcons:Item,
        skos:Concept,
        dcat:Resource ;
    rdfs:label "Item I1220"@en-AU ;
    rdfs:comment "234 AA  Places set aside for purposes of Act - GraphNodeID: I1220"@en-AU ;
    skos:definition "234 AA  Places set aside for purposes of Act"@en-AU ;
    skos:narrower C1901A00006:1162 ;
    skos:prefLabel "Item I1220"@en-AU ;
    dcat:accessURL "https://www.legislation.gov.au/C1901A00006/2024-07-01/2024-07-01/text/original/epub/OEBPS/document_3/document_3.html#_Toc172627254"^^xsd:anyURI .

C1901A00006:1221 a legcons:Item,
        skos:Concept,
        dcat:Resource ;
    rdfs:label "Item I1221"@en-AU ;
    rdfs:comment "234 A  Unauthorised entry to places and on ships aircraft or wharves - GraphNodeID: I1221"@en-AU ;
    skos:definition "234 A  Unauthorised entry to places and on ships aircraft or wharves"@en-AU ;
    skos:narrower C1901A00006:1162 ;
    skos:prefLabel "Item I1221"@en-AU ;
    dcat:accessURL "https://www.legislation.gov.au/C1901A00006/2024-07-01/2024-07-01/text/original/epub/OEBPS/document_3/document_3.html#_Toc172627255"^^xsd:anyURI .

C1901A00006:1222 a legcons:Item,
        skos:Concept,
        dcat:Resource ;
    rdfs:label "Item I1222"@en-AU ;
    rdfs:comment "234 AB  Unauthorised use of cameras and sound recorders - GraphNodeID: I1222"@en-AU ;
    skos:definition "234 AB  Unauthorised use of cameras and sound recorders"@en-AU ;
    skos:narrower C1901A00006:1162 ;
    skos:prefLabel "Item I1222"@en-AU ;
    dcat:accessURL "https://www.legislation.gov.au/C1901A00006/2024-07-01/2024-07-01/text/original/epub/OEBPS/document_3/document_3.html#_Toc172627256"^^xsd:anyURI .

C1901A00006:1223 a legcons:Item,
        skos:Concept,
        dcat:Resource ;
    rdfs:label "Item I1223"@en-AU ;
    rdfs:comment "234 ABA  Officers may direct unauthorised persons to leave restricted areas - GraphNodeID: I1223"@en-AU ;
    skos:definition "234 ABA  Officers may direct unauthorised persons to leave restricted areas"@en-AU ;
    skos:narrower C1901A00006:1162 ;
    skos:prefLabel "Item I1223"@en-AU ;
    dcat:accessURL "https://www.legislation.gov.au/C1901A00006/2024-07-01/2024-07-01/text/original/epub/OEBPS/document_3/document_3.html#_Toc172627257"^^xsd:anyURI .

C1901A00006:1224 a legcons:Item,
        skos:Concept,
        dcat:Resource ;
    rdfs:label "Item I1224"@en-AU ;
    rdfs:comment "236  Aiders and abettors - GraphNodeID: I1224"@en-AU ;
    skos:definition "236  Aiders and abettors"@en-AU ;
    skos:narrower C1901A00006:1162 ;
    skos:prefLabel "Item I1224"@en-AU ;
    dcat:accessURL "https://www.legislation.gov.au/C1901A00006/2024-07-01/2024-07-01/text/original/epub/OEBPS/document_3/document_3.html#_Toc172627258"^^xsd:anyURI .

C1901A00006:1225 a legcons:Item,
        skos:Concept,
        dcat:Resource ;
    rdfs:label "Item I1225"@en-AU ;
    rdfs:comment "237  Attempts - GraphNodeID: I1225"@en-AU ;
    skos:definition "237  Attempts"@en-AU ;
    skos:narrower C1901A00006:1162 ;
    skos:prefLabel "Item I1225"@en-AU ;
    dcat:accessURL "https://www.legislation.gov.au/C1901A00006/2024-07-01/2024-07-01/text/original/epub/OEBPS/document_3/document_3.html#_Toc172627259"^^xsd:anyURI .

C1901A00006:1226 a legcons:Item,
        skos:Concept,
        dcat:Resource ;
    rdfs:label "Item I1226"@en-AU ;
    rdfs:comment "239  Penalties in addition to forfeitures - GraphNodeID: I1226"@en-AU ;
    skos:definition "239  Penalties in addition to forfeitures"@en-AU ;
    skos:narrower C1901A00006:1162 ;
    skos:prefLabel "Item I1226"@en-AU ;
    dcat:accessURL "https://www.legislation.gov.au/C1901A00006/2024-07-01/2024-07-01/text/original/epub/OEBPS/document_3/document_3.html#_Toc172627260"^^xsd:anyURI .

C1901A00006:1227 a legcons:Item,
        skos:Concept,
        dcat:Resource ;
    rdfs:label "Item I1227"@en-AU ;
    rdfs:comment "240  Commercial documents to be kept - GraphNodeID: I1227"@en-AU ;
    skos:definition "240  Commercial documents to be kept"@en-AU ;
    skos:narrower C1901A00006:1162 ;
    skos:prefLabel "Item I1227"@en-AU ;
    dcat:accessURL "https://www.legislation.gov.au/C1901A00006/2024-07-01/2024-07-01/text/original/epub/OEBPS/document_3/document_3.html#_Toc172627261"^^xsd:anyURI .

C1901A00006:1228 a legcons:Item,
        skos:Concept,
        dcat:Resource ;
    rdfs:label "Item I1228"@en-AU ;
    rdfs:comment "240 AA  Authorised officer may require person to produce commercial documents - GraphNodeID: I1228"@en-AU ;
    skos:definition "240 AA  Authorised officer may require person to produce commercial documents"@en-AU ;
    skos:narrower C1901A00006:1162 ;
    skos:prefLabel "Item I1228"@en-AU ;
    dcat:accessURL "https://www.legislation.gov.au/C1901A00006/2024-07-01/2024-07-01/text/original/epub/OEBPS/document_3/document_3.html#_Toc172627262"^^xsd:anyURI .

C1901A00006:1229 a legcons:Item,
        skos:Concept,
        dcat:Resource ;
    rdfs:label "Item I1229"@en-AU ;
    rdfs:comment "240 AB  Verifying communications to Department - GraphNodeID: I1229"@en-AU ;
    skos:definition "240 AB  Verifying communications to Department"@en-AU ;
    skos:narrower C1901A00006:1162 ;
    skos:prefLabel "Item I1229"@en-AU ;
    dcat:accessURL "https://www.legislation.gov.au/C1901A00006/2024-07-01/2024-07-01/text/original/epub/OEBPS/document_3/document_3.html#_Toc172627263"^^xsd:anyURI .

C1901A00006:123 a legcons:Item,
        skos:Concept,
        dcat:Resource ;
    rdfs:label "Item I123"@en-AU ;
    rdfs:comment "68 A  Goods imported for transhipment - GraphNodeID: I123"@en-AU ;
    skos:definition "68 A  Goods imported for transhipment"@en-AU ;
    skos:narrower C1901A00006:121 ;
    skos:prefLabel "Item I123"@en-AU ;
    dcat:accessURL "https://www.legislation.gov.au/C1901A00006/2024-07-01/2024-07-01/text/original/epub/OEBPS/document_1/document_1.html#_Toc172623097"^^xsd:anyURI .

C1901A00006:1230 a legcons:Item,
        skos:Concept,
        dcat:Resource ;
    rdfs:label "Item I1230"@en-AU ;
    rdfs:comment "240 AC  Authorised officer may require person to produce record - GraphNodeID: I1230"@en-AU ;
    skos:definition "240 AC  Authorised officer may require person to produce record"@en-AU ;
    skos:narrower C1901A00006:1162 ;
    skos:prefLabel "Item I1230"@en-AU ;
    dcat:accessURL "https://www.legislation.gov.au/C1901A00006/2024-07-01/2024-07-01/text/original/epub/OEBPS/document_3/document_3.html#_Toc172627264"^^xsd:anyURI .

C1901A00006:1231 a legcons:Division,
        skos:Concept,
        dcat:Resource ;
    rdfs:label "Division D1231"@en-AU ;
    rdfs:comment "Division 3 Recovery of pecuniary penalties for dealings in narcotic goods - GraphNodeID: D1231"@en-AU ;
    skos:definition "Division 3 Recovery of pecuniary penalties for dealings in narcotic goods"@en-AU ;
    skos:narrower C1901A00006:1192 ;
    skos:prefLabel "Division D1231"@en-AU ;
    dcat:accessURL "https://www.legislation.gov.au/C1901A00006/2024-07-01/2024-07-01/text/original/epub/OEBPS/document_3/document_3.html#_Toc172627265"^^xsd:anyURI .

C1901A00006:1232 a legcons:Item,
        skos:Concept,
        dcat:Resource ;
    rdfs:label "Item I1232"@en-AU ;
    rdfs:comment "243 A  Interpretation - GraphNodeID: I1232"@en-AU ;
    skos:definition "243 A  Interpretation"@en-AU ;
    skos:narrower C1901A00006:1162 ;
    skos:prefLabel "Item I1232"@en-AU ;
    dcat:accessURL "https://www.legislation.gov.au/C1901A00006/2024-07-01/2024-07-01/text/original/epub/OEBPS/document_3/document_3.html#_Toc172627266"^^xsd:anyURI .

C1901A00006:1233 a legcons:Item,
        skos:Concept,
        dcat:Resource ;
    rdfs:label "Item I1233"@en-AU ;
    rdfs:comment "243 AB  Effective control of property - GraphNodeID: I1233"@en-AU ;
    skos:definition "243 AB  Effective control of property"@en-AU ;
    skos:narrower C1901A00006:1162 ;
    skos:prefLabel "Item I1233"@en-AU ;
    dcat:accessURL "https://www.legislation.gov.au/C1901A00006/2024-07-01/2024-07-01/text/original/epub/OEBPS/document_3/document_3.html#_Toc172627267"^^xsd:anyURI .

C1901A00006:1234 a legcons:Item,
        skos:Concept,
        dcat:Resource ;
    rdfs:label "Item I1234"@en-AU ;
    rdfs:comment "243 B  Pecuniary penalties - GraphNodeID: I1234"@en-AU ;
    skos:definition "243 B  Pecuniary penalties"@en-AU ;
    skos:narrower C1901A00006:1162 ;
    skos:prefLabel "Item I1234"@en-AU ;
    dcat:accessURL "https://www.legislation.gov.au/C1901A00006/2024-07-01/2024-07-01/text/original/epub/OEBPS/document_3/document_3.html#_Toc172627268"^^xsd:anyURI .

C1901A00006:1235 a legcons:Item,
        skos:Concept,
        dcat:Resource ;
    rdfs:label "Item I1235"@en-AU ;
    rdfs:comment "243 C  Assessment of pecuniary penalty - GraphNodeID: I1235"@en-AU ;
    skos:definition "243 C  Assessment of pecuniary penalty"@en-AU ;
    skos:narrower C1901A00006:1162 ;
    skos:prefLabel "Item I1235"@en-AU ;
    dcat:accessURL "https://www.legislation.gov.au/C1901A00006/2024-07-01/2024-07-01/text/original/epub/OEBPS/document_3/document_3.html#_Toc172627269"^^xsd:anyURI .

C1901A00006:1236 a legcons:Item,
        skos:Concept,
        dcat:Resource ;
    rdfs:label "Item I1236"@en-AU ;
    rdfs:comment "243 CA  Court may lift corporate veil etc - GraphNodeID: I1236"@en-AU ;
    skos:definition "243 CA  Court may lift corporate veil etc"@en-AU ;
    skos:narrower C1901A00006:1162 ;
    skos:prefLabel "Item I1236"@en-AU ;
    dcat:accessURL "https://www.legislation.gov.au/C1901A00006/2024-07-01/2024-07-01/text/original/epub/OEBPS/document_3/document_3.html#_Toc172627270"^^xsd:anyURI .

C1901A00006:1237 a legcons:Item,
        skos:Concept,
        dcat:Resource ;
    rdfs:label "Item I1237"@en-AU ;
    rdfs:comment "243 D  Presumption of illegality of importation - GraphNodeID: I1237"@en-AU ;
    skos:definition "243 D  Presumption of illegality of importation"@en-AU ;
    skos:narrower C1901A00006:1162 ;
    skos:prefLabel "Item I1237"@en-AU ;
    dcat:accessURL "https://www.legislation.gov.au/C1901A00006/2024-07-01/2024-07-01/text/original/epub/OEBPS/document_3/document_3.html#_Toc172627271"^^xsd:anyURI .

C1901A00006:1238 a legcons:Item,
        skos:Concept,
        dcat:Resource ;
    rdfs:label "Item I1238"@en-AU ;
    rdfs:comment "243 E  Court may make restraining order against property - GraphNodeID: I1238"@en-AU ;
    skos:definition "243 E  Court may make restraining order against property"@en-AU ;
    skos:narrower C1901A00006:1162 ;
    skos:prefLabel "Item I1238"@en-AU ;
    dcat:accessURL "https://www.legislation.gov.au/C1901A00006/2024-07-01/2024-07-01/text/original/epub/OEBPS/document_3/document_3.html#_Toc172627272"^^xsd:anyURI .

C1901A00006:1239 a legcons:Item,
        skos:Concept,
        dcat:Resource ;
    rdfs:label "Item I1239"@en-AU ;
    rdfs:comment "243 F  Court may make further orders - GraphNodeID: I1239"@en-AU ;
    skos:definition "243 F  Court may make further orders"@en-AU ;
    skos:narrower C1901A00006:1162 ;
    skos:prefLabel "Item I1239"@en-AU ;
    dcat:accessURL "https://www.legislation.gov.au/C1901A00006/2024-07-01/2024-07-01/text/original/epub/OEBPS/document_3/document_3.html#_Toc172627273"^^xsd:anyURI .

C1901A00006:124 a legcons:Item,
        skos:Concept,
        dcat:Resource ;
    rdfs:label "Item I124"@en-AU ;
    rdfs:comment "69  Like customable goods and excise equivalent goods - GraphNodeID: I124"@en-AU ;
    skos:definition "69  Like customable goods and excise equivalent goods"@en-AU ;
    skos:narrower C1901A00006:121 ;
    skos:prefLabel "Item I124"@en-AU ;
    dcat:accessURL "https://www.legislation.gov.au/C1901A00006/2024-07-01/2024-07-01/text/original/epub/OEBPS/document_1/document_1.html#_Toc172623098"^^xsd:anyURI .

C1901A00006:1240 a legcons:Item,
        skos:Concept,
        dcat:Resource ;
    rdfs:label "Item I1240"@en-AU ;
    rdfs:comment "243 G  Official Trustee to discharge pecuniary penalty - GraphNodeID: I1240"@en-AU ;
    skos:definition "243 G  Official Trustee to discharge pecuniary penalty"@en-AU ;
    skos:narrower C1901A00006:1162 ;
    skos:prefLabel "Item I1240"@en-AU ;
    dcat:accessURL "https://www.legislation.gov.au/C1901A00006/2024-07-01/2024-07-01/text/original/epub/OEBPS/document_3/document_3.html#_Toc172627274"^^xsd:anyURI .

C1901A00006:1241 a legcons:Item,
        skos:Concept,
        dcat:Resource ;
    rdfs:label "Item I1241"@en-AU ;
    rdfs:comment "243 H  Revocation of order under section 243 E - GraphNodeID: I1241"@en-AU ;
    skos:definition "243 H  Revocation of order under section 243 E"@en-AU ;
    skos:narrower C1901A00006:1162 ;
    skos:prefLabel "Item I1241"@en-AU ;
    dcat:accessURL "https://www.legislation.gov.au/C1901A00006/2024-07-01/2024-07-01/text/original/epub/OEBPS/document_3/document_3.html#_Toc172627275"^^xsd:anyURI .

C1901A00006:1242 a legcons:Item,
        skos:Concept,
        dcat:Resource ;
    rdfs:label "Item I1242"@en-AU ;
    rdfs:comment "243 J  Pecuniary penalty a charge on property - GraphNodeID: I1242"@en-AU ;
    skos:definition "243 J  Pecuniary penalty a charge on property"@en-AU ;
    skos:narrower C1901A00006:1162 ;
    skos:prefLabel "Item I1242"@en-AU ;
    dcat:accessURL "https://www.legislation.gov.au/C1901A00006/2024-07-01/2024-07-01/text/original/epub/OEBPS/document_3/document_3.html#_Toc172627276"^^xsd:anyURI .

C1901A00006:1243 a legcons:Item,
        skos:Concept,
        dcat:Resource ;
    rdfs:label "Item I1243"@en-AU ;
    rdfs:comment "243 K  Contravention of restraining orders - GraphNodeID: I1243"@en-AU ;
    skos:definition "243 K  Contravention of restraining orders"@en-AU ;
    skos:narrower C1901A00006:1162 ;
    skos:prefLabel "Item I1243"@en-AU ;
    dcat:accessURL "https://www.legislation.gov.au/C1901A00006/2024-07-01/2024-07-01/text/original/epub/OEBPS/document_3/document_3.html#_Toc172627277"^^xsd:anyURI .

C1901A00006:1244 a legcons:Item,
        skos:Concept,
        dcat:Resource ;
    rdfs:label "Item I1244"@en-AU ;
    rdfs:comment "243 L  Sale of property before bankruptcy - GraphNodeID: I1244"@en-AU ;
    skos:definition "243 L  Sale of property before bankruptcy"@en-AU ;
    skos:narrower C1901A00006:1162 ;
    skos:prefLabel "Item I1244"@en-AU ;
    dcat:accessURL "https://www.legislation.gov.au/C1901A00006/2024-07-01/2024-07-01/text/original/epub/OEBPS/document_3/document_3.html#_Toc172627278"^^xsd:anyURI .

C1901A00006:1245 a legcons:Item,
        skos:Concept,
        dcat:Resource ;
    rdfs:label "Item I1245"@en-AU ;
    rdfs:comment "243 M  Duties of the Official Trustee after receiving notice of presentation of creditors petition etc - GraphNodeID: I1245"@en-AU ;
    skos:definition "243 M  Duties of the Official Trustee after receiving notice of presentation of creditors petition etc"@en-AU ;
    skos:narrower C1901A00006:1162 ;
    skos:prefLabel "Item I1245"@en-AU ;
    dcat:accessURL "https://www.legislation.gov.au/C1901A00006/2024-07-01/2024-07-01/text/original/epub/OEBPS/document_3/document_3.html#_Toc172627279"^^xsd:anyURI .

C1901A00006:1246 a legcons:Item,
        skos:Concept,
        dcat:Resource ;
    rdfs:label "Item I1246"@en-AU ;
    rdfs:comment "243 N  Protection of Official Trustee from personal liability in certain cases - GraphNodeID: I1246"@en-AU ;
    skos:definition "243 N  Protection of Official Trustee from personal liability in certain cases"@en-AU ;
    skos:narrower C1901A00006:1162 ;
    skos:prefLabel "Item I1246"@en-AU ;
    dcat:accessURL "https://www.legislation.gov.au/C1901A00006/2024-07-01/2024-07-01/text/original/epub/OEBPS/document_3/document_3.html#_Toc172627280"^^xsd:anyURI .

C1901A00006:1247 a legcons:Item,
        skos:Concept,
        dcat:Resource ;
    rdfs:label "Item I1247"@en-AU ;
    rdfs:comment "243 NA  Indemnification of Official Trustee - GraphNodeID: I1247"@en-AU ;
    skos:definition "243 NA  Indemnification of Official Trustee"@en-AU ;
    skos:narrower C1901A00006:1162 ;
    skos:prefLabel "Item I1247"@en-AU ;
    dcat:accessURL "https://www.legislation.gov.au/C1901A00006/2024-07-01/2024-07-01/text/original/epub/OEBPS/document_3/document_3.html#_Toc172627281"^^xsd:anyURI .

C1901A00006:1248 a legcons:Item,
        skos:Concept,
        dcat:Resource ;
    rdfs:label "Item I1248"@en-AU ;
    rdfs:comment "243 NB  Indemnification of Official Receivers etc - GraphNodeID: I1248"@en-AU ;
    skos:definition "243 NB  Indemnification of Official Receivers etc"@en-AU ;
    skos:narrower C1901A00006:1162 ;
    skos:prefLabel "Item I1248"@en-AU ;
    dcat:accessURL "https://www.legislation.gov.au/C1901A00006/2024-07-01/2024-07-01/text/original/epub/OEBPS/document_3/document_3.html#_Toc172627282"^^xsd:anyURI .

C1901A00006:1249 a legcons:Item,
        skos:Concept,
        dcat:Resource ;
    rdfs:label "Item I1249"@en-AU ;
    rdfs:comment "243 P  Costs etc payable to Official Trustee - GraphNodeID: I1249"@en-AU ;
    skos:definition "243 P  Costs etc payable to Official Trustee"@en-AU ;
    skos:narrower C1901A00006:1162 ;
    skos:prefLabel "Item I1249"@en-AU ;
    dcat:accessURL "https://www.legislation.gov.au/C1901A00006/2024-07-01/2024-07-01/text/original/epub/OEBPS/document_3/document_3.html#_Toc172627283"^^xsd:anyURI .

C1901A00006:125 a legcons:Item,
        skos:Concept,
        dcat:Resource ;
    rdfs:label "Item I125"@en-AU ;
    rdfs:comment "70  Special clearance goods - GraphNodeID: I125"@en-AU ;
    skos:definition "70  Special clearance goods"@en-AU ;
    skos:narrower C1901A00006:121 ;
    skos:prefLabel "Item I125"@en-AU ;
    dcat:accessURL "https://www.legislation.gov.au/C1901A00006/2024-07-01/2024-07-01/text/original/epub/OEBPS/document_1/document_1.html#_Toc172623099"^^xsd:anyURI .

C1901A00006:1250 a legcons:Item,
        skos:Concept,
        dcat:Resource ;
    rdfs:label "Item I1250"@en-AU ;
    rdfs:comment "243 Q  Notices - GraphNodeID: I1250"@en-AU ;
    skos:definition "243 Q  Notices"@en-AU ;
    skos:narrower C1901A00006:1162 ;
    skos:prefLabel "Item I1250"@en-AU ;
    dcat:accessURL "https://www.legislation.gov.au/C1901A00006/2024-07-01/2024-07-01/text/original/epub/OEBPS/document_3/document_3.html#_Toc172627284"^^xsd:anyURI .

C1901A00006:1251 a legcons:Item,
        skos:Concept,
        dcat:Resource ;
    rdfs:label "Item I1251"@en-AU ;
    rdfs:comment "243 R  Reduction of pecuniary penalty - GraphNodeID: I1251"@en-AU ;
    skos:definition "243 R  Reduction of pecuniary penalty"@en-AU ;
    skos:narrower C1901A00006:1162 ;
    skos:prefLabel "Item I1251"@en-AU ;
    dcat:accessURL "https://www.legislation.gov.au/C1901A00006/2024-07-01/2024-07-01/text/original/epub/OEBPS/document_3/document_3.html#_Toc172627285"^^xsd:anyURI .

C1901A00006:1252 a legcons:Item,
        skos:Concept,
        dcat:Resource ;
    rdfs:label "Item I1252"@en-AU ;
    rdfs:comment "243 S  Jurisdiction of the Court - GraphNodeID: I1252"@en-AU ;
    skos:definition "243 S  Jurisdiction of the Court"@en-AU ;
    skos:narrower C1901A00006:1162 ;
    skos:prefLabel "Item I1252"@en-AU ;
    dcat:accessURL "https://www.legislation.gov.au/C1901A00006/2024-07-01/2024-07-01/text/original/epub/OEBPS/document_3/document_3.html#_Toc172627286"^^xsd:anyURI .

C1901A00006:1253 a legcons:Division,
        skos:Concept,
        dcat:Resource ;
    rdfs:label "Division D1253"@en-AU ;
    rdfs:comment "Division 4 Provisions relating to certain strict liability offences - GraphNodeID: D1253"@en-AU ;
    skos:definition "Division 4 Provisions relating to certain strict liability offences"@en-AU ;
    skos:narrower C1901A00006:1192 ;
    skos:prefLabel "Division D1253"@en-AU ;
    dcat:accessURL "https://www.legislation.gov.au/C1901A00006/2024-07-01/2024-07-01/text/original/epub/OEBPS/document_3/document_3.html#_Toc172627287"^^xsd:anyURI .

C1901A00006:1254 a legcons:Item,
        skos:Concept,
        dcat:Resource ;
    rdfs:label "Item I1254"@en-AU ;
    rdfs:comment "243 SA  Failure to answer questions - GraphNodeID: I1254"@en-AU ;
    skos:definition "243 SA  Failure to answer questions"@en-AU ;
    skos:narrower C1901A00006:1162 ;
    skos:prefLabel "Item I1254"@en-AU ;
    dcat:accessURL "https://www.legislation.gov.au/C1901A00006/2024-07-01/2024-07-01/text/original/epub/OEBPS/document_3/document_3.html#_Toc172627288"^^xsd:anyURI .

C1901A00006:1255 a legcons:Item,
        skos:Concept,
        dcat:Resource ;
    rdfs:label "Item I1255"@en-AU ;
    rdfs:comment "243 SB  Failure to produce documents or records - GraphNodeID: I1255"@en-AU ;
    skos:definition "243 SB  Failure to produce documents or records"@en-AU ;
    skos:narrower C1901A00006:1162 ;
    skos:prefLabel "Item I1255"@en-AU ;
    dcat:accessURL "https://www.legislation.gov.au/C1901A00006/2024-07-01/2024-07-01/text/original/epub/OEBPS/document_3/document_3.html#_Toc172627289"^^xsd:anyURI .

C1901A00006:1256 a legcons:Item,
        skos:Concept,
        dcat:Resource ;
    rdfs:label "Item I1256"@en-AU ;
    rdfs:comment "243 SC  Preservation of the privilege against self incrimination - GraphNodeID: I1256"@en-AU ;
    skos:definition "243 SC  Preservation of the privilege against self incrimination"@en-AU ;
    skos:narrower C1901A00006:1162 ;
    skos:prefLabel "Item I1256"@en-AU ;
    dcat:accessURL "https://www.legislation.gov.au/C1901A00006/2024-07-01/2024-07-01/text/original/epub/OEBPS/document_3/document_3.html#_Toc172627290"^^xsd:anyURI .

C1901A00006:1257 a legcons:Item,
        skos:Concept,
        dcat:Resource ;
    rdfs:label "Item I1257"@en-AU ;
    rdfs:comment "243 T  False or misleading statements resulting in loss of duty - GraphNodeID: I1257"@en-AU ;
    skos:definition "243 T  False or misleading statements resulting in loss of duty"@en-AU ;
    skos:narrower C1901A00006:1162 ;
    skos:prefLabel "Item I1257"@en-AU ;
    dcat:accessURL "https://www.legislation.gov.au/C1901A00006/2024-07-01/2024-07-01/text/original/epub/OEBPS/document_3/document_3.html#_Toc172627291"^^xsd:anyURI .

C1901A00006:1258 a legcons:Item,
        skos:Concept,
        dcat:Resource ;
    rdfs:label "Item I1258"@en-AU ;
    rdfs:comment "243 U  False or misleading statements not resulting in loss of duty - GraphNodeID: I1258"@en-AU ;
    skos:definition "243 U  False or misleading statements not resulting in loss of duty"@en-AU ;
    skos:narrower C1901A00006:1162 ;
    skos:prefLabel "Item I1258"@en-AU ;
    dcat:accessURL "https://www.legislation.gov.au/C1901A00006/2024-07-01/2024-07-01/text/original/epub/OEBPS/document_3/document_3.html#_Toc172627292"^^xsd:anyURI .

C1901A00006:1259 a legcons:Item,
        skos:Concept,
        dcat:Resource ;
    rdfs:label "Item I1259"@en-AU ;
    rdfs:comment "243 V  False or misleading statements in cargo reports or outturn reports - GraphNodeID: I1259"@en-AU ;
    skos:definition "243 V  False or misleading statements in cargo reports or outturn reports"@en-AU ;
    skos:narrower C1901A00006:1162 ;
    skos:prefLabel "Item I1259"@en-AU ;
    dcat:accessURL "https://www.legislation.gov.au/C1901A00006/2024-07-01/2024-07-01/text/original/epub/OEBPS/document_3/document_3.html#_Toc172627293"^^xsd:anyURI .

C1901A00006:126 a legcons:Item,
        skos:Concept,
        dcat:Resource ;
    rdfs:label "Item I126"@en-AU ;
    rdfs:comment "71  Information and grant of authority to deal with goods not required to be entered - GraphNodeID: I126"@en-AU ;
    skos:definition "71  Information and grant of authority to deal with goods not required to be entered"@en-AU ;
    skos:narrower C1901A00006:121 ;
    skos:prefLabel "Item I126"@en-AU ;
    dcat:accessURL "https://www.legislation.gov.au/C1901A00006/2024-07-01/2024-07-01/text/original/epub/OEBPS/document_1/document_1.html#_Toc172623100"^^xsd:anyURI .

C1901A00006:1260 a legcons:Item,
        skos:Concept,
        dcat:Resource ;
    rdfs:label "Item I1260"@en-AU ;
    rdfs:comment "243 W  Electronic communications to Department to be treated as statements to Comptroller General of Customs - GraphNodeID: I1260"@en-AU ;
    skos:definition "243 W  Electronic communications to Department to be treated as statements to Comptroller General of Customs"@en-AU ;
    skos:narrower C1901A00006:1162 ;
    skos:prefLabel "Item I1260"@en-AU ;
    dcat:accessURL "https://www.legislation.gov.au/C1901A00006/2024-07-01/2024-07-01/text/original/epub/OEBPS/document_3/document_3.html#_Toc172627294"^^xsd:anyURI .

C1901A00006:1261 a legcons:Division,
        skos:Concept,
        dcat:Resource ;
    rdfs:label "Division D1261"@en-AU ;
    rdfs:comment "Division 5 Infringement notices - GraphNodeID: D1261"@en-AU ;
    skos:definition "Division 5 Infringement notices"@en-AU ;
    skos:narrower C1901A00006:1192 ;
    skos:prefLabel "Division D1261"@en-AU ;
    dcat:accessURL "https://www.legislation.gov.au/C1901A00006/2024-07-01/2024-07-01/text/original/epub/OEBPS/document_3/document_3.html#_Toc172627295"^^xsd:anyURI .

C1901A00006:1262 a legcons:Item,
        skos:Concept,
        dcat:Resource ;
    rdfs:label "Item I1262"@en-AU ;
    rdfs:comment "243 X  Infringement noticesgeneral - GraphNodeID: I1262"@en-AU ;
    skos:definition "243 X  Infringement noticesgeneral"@en-AU ;
    skos:narrower C1901A00006:1162 ;
    skos:prefLabel "Item I1262"@en-AU ;
    dcat:accessURL "https://www.legislation.gov.au/C1901A00006/2024-07-01/2024-07-01/text/original/epub/OEBPS/document_3/document_3.html#_Toc172627296"^^xsd:anyURI .

C1901A00006:1263 a legcons:Item,
        skos:Concept,
        dcat:Resource ;
    rdfs:label "Item I1263"@en-AU ;
    rdfs:comment "243 Y  Infringement noticesforfeiture of goods that are prohibited imports if infringement notice paid - GraphNodeID: I1263"@en-AU ;
    skos:definition "243 Y  Infringement noticesforfeiture of goods that are prohibited imports if infringement notice paid"@en-AU ;
    skos:narrower C1901A00006:1162 ;
    skos:prefLabel "Item I1263"@en-AU ;
    dcat:accessURL "https://www.legislation.gov.au/C1901A00006/2024-07-01/2024-07-01/text/original/epub/OEBPS/document_3/document_3.html#_Toc172627297"^^xsd:anyURI .

C1901A00006:1264 a legcons:Item,
        skos:Concept,
        dcat:Resource ;
    rdfs:label "Item I1264"@en-AU ;
    rdfs:comment "243 Z  Infringement noticesright of compensation in certain circumstances for goods disposed of or destroyed - GraphNodeID: I1264"@en-AU ;
    skos:definition "243 Z  Infringement noticesright of compensation in certain circumstances for goods disposed of or destroyed"@en-AU ;
    skos:narrower C1901A00006:1162 ;
    skos:prefLabel "Item I1264"@en-AU ;
    dcat:accessURL "https://www.legislation.gov.au/C1901A00006/2024-07-01/2024-07-01/text/original/epub/OEBPS/document_3/document_3.html#_Toc172627298"^^xsd:anyURI .

C1901A00006:1265 a legcons:Part,
        skos:Concept,
        dcat:Resource ;
    rdfs:label "Part P1265"@en-AU ;
    rdfs:comment "Part XIVCustoms prosecutions - GraphNodeID: P1265"@en-AU ;
    skos:definition "Part XIVCustoms prosecutions"@en-AU ;
    skos:narrower C1901A00006:952 ;
    skos:prefLabel "Part P1265"@en-AU ;
    dcat:accessURL "https://www.legislation.gov.au/C1901A00006/2024-07-01/2024-07-01/text/original/epub/OEBPS/document_3/document_3.html#_Toc172627299"^^xsd:anyURI .

C1901A00006:1266 a legcons:Item,
        skos:Concept,
        dcat:Resource ;
    rdfs:label "Item I1266"@en-AU ;
    rdfs:comment "244  Meaning of Customs prosecution - GraphNodeID: I1266"@en-AU ;
    skos:definition "244  Meaning of Customs prosecution"@en-AU ;
    skos:narrower C1901A00006:1162 ;
    skos:prefLabel "Item I1266"@en-AU ;
    dcat:accessURL "https://www.legislation.gov.au/C1901A00006/2024-07-01/2024-07-01/text/original/epub/OEBPS/document_3/document_3.html#_Toc172627300"^^xsd:anyURI .

C1901A00006:1267 a legcons:Item,
        skos:Concept,
        dcat:Resource ;
    rdfs:label "Item I1267"@en-AU ;
    rdfs:comment "245  Institution of prosecutions - GraphNodeID: I1267"@en-AU ;
    skos:definition "245  Institution of prosecutions"@en-AU ;
    skos:narrower C1901A00006:1162 ;
    skos:prefLabel "Item I1267"@en-AU ;
    dcat:accessURL "https://www.legislation.gov.au/C1901A00006/2024-07-01/2024-07-01/text/original/epub/OEBPS/document_3/document_3.html#_Toc172627301"^^xsd:anyURI .

C1901A00006:1268 a legcons:Item,
        skos:Concept,
        dcat:Resource ;
    rdfs:label "Item I1268"@en-AU ;
    rdfs:comment "247  Prosecutions in accordance with practice rules - GraphNodeID: I1268"@en-AU ;
    skos:definition "247  Prosecutions in accordance with practice rules"@en-AU ;
    skos:narrower C1901A00006:1162 ;
    skos:prefLabel "Item I1268"@en-AU ;
    dcat:accessURL "https://www.legislation.gov.au/C1901A00006/2024-07-01/2024-07-01/text/original/epub/OEBPS/document_3/document_3.html#_Toc172627302"^^xsd:anyURI .

C1901A00006:1269 a legcons:Item,
        skos:Concept,
        dcat:Resource ;
    rdfs:label "Item I1269"@en-AU ;
    rdfs:comment "248  State Court practice - GraphNodeID: I1269"@en-AU ;
    skos:definition "248  State Court practice"@en-AU ;
    skos:narrower C1901A00006:1162 ;
    skos:prefLabel "Item I1269"@en-AU ;
    dcat:accessURL "https://www.legislation.gov.au/C1901A00006/2024-07-01/2024-07-01/text/original/epub/OEBPS/document_3/document_3.html#_Toc172627303"^^xsd:anyURI .

C1901A00006:1270 a legcons:Item,
        skos:Concept,
        dcat:Resource ;
    rdfs:label "Item I1270"@en-AU ;
    rdfs:comment "249  Commencement of prosecutions - GraphNodeID: I1270"@en-AU ;
    skos:definition "249  Commencement of prosecutions"@en-AU ;
    skos:narrower C1901A00006:1162 ;
    skos:prefLabel "Item I1270"@en-AU ;
    dcat:accessURL "https://www.legislation.gov.au/C1901A00006/2024-07-01/2024-07-01/text/original/epub/OEBPS/document_3/document_3.html#_Toc172627304"^^xsd:anyURI .

C1901A00006:1271 a legcons:Item,
        skos:Concept,
        dcat:Resource ;
    rdfs:label "Item I1271"@en-AU ;
    rdfs:comment "250  Information to be valid if in words of Act - GraphNodeID: I1271"@en-AU ;
    skos:definition "250  Information to be valid if in words of Act"@en-AU ;
    skos:narrower C1901A00006:1162 ;
    skos:prefLabel "Item I1271"@en-AU ;
    dcat:accessURL "https://www.legislation.gov.au/C1901A00006/2024-07-01/2024-07-01/text/original/epub/OEBPS/document_3/document_3.html#_Toc172627305"^^xsd:anyURI .

C1901A00006:1272 a legcons:Item,
        skos:Concept,
        dcat:Resource ;
    rdfs:label "Item I1272"@en-AU ;
    rdfs:comment "250 A  Property in goods subject to customs control - GraphNodeID: I1272"@en-AU ;
    skos:definition "250 A  Property in goods subject to customs control"@en-AU ;
    skos:narrower C1901A00006:1162 ;
    skos:prefLabel "Item I1272"@en-AU ;
    dcat:accessURL "https://www.legislation.gov.au/C1901A00006/2024-07-01/2024-07-01/text/original/epub/OEBPS/document_3/document_3.html#_Toc172627306"^^xsd:anyURI .

C1901A00006:1273 a legcons:Item,
        skos:Concept,
        dcat:Resource ;
    rdfs:label "Item I1273"@en-AU ;
    rdfs:comment "251  No objection for informality - GraphNodeID: I1273"@en-AU ;
    skos:definition "251  No objection for informality"@en-AU ;
    skos:narrower C1901A00006:1162 ;
    skos:prefLabel "Item I1273"@en-AU ;
    dcat:accessURL "https://www.legislation.gov.au/C1901A00006/2024-07-01/2024-07-01/text/original/epub/OEBPS/document_3/document_3.html#_Toc172627307"^^xsd:anyURI .

C1901A00006:1274 a legcons:Item,
        skos:Concept,
        dcat:Resource ;
    rdfs:label "Item I1274"@en-AU ;
    rdfs:comment "252  Conviction not to be quashed - GraphNodeID: I1274"@en-AU ;
    skos:definition "252  Conviction not to be quashed"@en-AU ;
    skos:narrower C1901A00006:1162 ;
    skos:prefLabel "Item I1274"@en-AU ;
    dcat:accessURL "https://www.legislation.gov.au/C1901A00006/2024-07-01/2024-07-01/text/original/epub/OEBPS/document_3/document_3.html#_Toc172627308"^^xsd:anyURI .

C1901A00006:1275 a legcons:Item,
        skos:Concept,
        dcat:Resource ;
    rdfs:label "Item I1275"@en-AU ;
    rdfs:comment "253  Protection to witnesses - GraphNodeID: I1275"@en-AU ;
    skos:definition "253  Protection to witnesses"@en-AU ;
    skos:narrower C1901A00006:1162 ;
    skos:prefLabel "Item I1275"@en-AU ;
    dcat:accessURL "https://www.legislation.gov.au/C1901A00006/2024-07-01/2024-07-01/text/original/epub/OEBPS/document_3/document_3.html#_Toc172627309"^^xsd:anyURI .

C1901A00006:1276 a legcons:Item,
        skos:Concept,
        dcat:Resource ;
    rdfs:label "Item I1276"@en-AU ;
    rdfs:comment "254  Defendant competent witness - GraphNodeID: I1276"@en-AU ;
    skos:definition "254  Defendant competent witness"@en-AU ;
    skos:narrower C1901A00006:1162 ;
    skos:prefLabel "Item I1276"@en-AU ;
    dcat:accessURL "https://www.legislation.gov.au/C1901A00006/2024-07-01/2024-07-01/text/original/epub/OEBPS/document_3/document_3.html#_Toc172627310"^^xsd:anyURI .

C1901A00006:1277 a legcons:Item,
        skos:Concept,
        dcat:Resource ;
    rdfs:label "Item I1277"@en-AU ;
    rdfs:comment "255  Averment of prosecutor sufficient - GraphNodeID: I1277"@en-AU ;
    skos:definition "255  Averment of prosecutor sufficient"@en-AU ;
    skos:narrower C1901A00006:1162 ;
    skos:prefLabel "Item I1277"@en-AU ;
    dcat:accessURL "https://www.legislation.gov.au/C1901A00006/2024-07-01/2024-07-01/text/original/epub/OEBPS/document_3/document_3.html#_Toc172627311"^^xsd:anyURI .

C1901A00006:1278 a legcons:Item,
        skos:Concept,
        dcat:Resource ;
    rdfs:label "Item I1278"@en-AU ;
    rdfs:comment "256  Proof of proclamation etc - GraphNodeID: I1278"@en-AU ;
    skos:definition "256  Proof of proclamation etc"@en-AU ;
    skos:narrower C1901A00006:1162 ;
    skos:prefLabel "Item I1278"@en-AU ;
    dcat:accessURL "https://www.legislation.gov.au/C1901A00006/2024-07-01/2024-07-01/text/original/epub/OEBPS/document_3/document_3.html#_Toc172627312"^^xsd:anyURI .

C1901A00006:1279 a legcons:Item,
        skos:Concept,
        dcat:Resource ;
    rdfs:label "Item I1279"@en-AU ;
    rdfs:comment "257  Conduct by directors employees or agents - GraphNodeID: I1279"@en-AU ;
    skos:definition "257  Conduct by directors employees or agents"@en-AU ;
    skos:narrower C1901A00006:1162 ;
    skos:prefLabel "Item I1279"@en-AU ;
    dcat:accessURL "https://www.legislation.gov.au/C1901A00006/2024-07-01/2024-07-01/text/original/epub/OEBPS/document_3/document_3.html#_Toc172627313"^^xsd:anyURI .

C1901A00006:128 a legcons:Item,
        skos:Concept,
        dcat:Resource ;
    rdfs:label "Item I128"@en-AU ;
    rdfs:comment "71 AAAA  Meaning of Subdivision AA goods - GraphNodeID: I128"@en-AU ;
    skos:definition "71 AAAA  Meaning of Subdivision AA goods"@en-AU ;
    skos:narrower C1901A00006:127 ;
    skos:prefLabel "Item I128"@en-AU ;
    dcat:accessURL "https://www.legislation.gov.au/C1901A00006/2024-07-01/2024-07-01/text/original/epub/OEBPS/document_1/document_1.html#_Toc172623102"^^xsd:anyURI .

C1901A00006:1280 a legcons:Item,
        skos:Concept,
        dcat:Resource ;
    rdfs:label "Item I1280"@en-AU ;
    rdfs:comment "259  Collector may levy on goods in his or her possession - GraphNodeID: I1280"@en-AU ;
    skos:definition "259  Collector may levy on goods in his or her possession"@en-AU ;
    skos:narrower C1901A00006:1162 ;
    skos:prefLabel "Item I1280"@en-AU ;
    dcat:accessURL "https://www.legislation.gov.au/C1901A00006/2024-07-01/2024-07-01/text/original/epub/OEBPS/document_3/document_3.html#_Toc172627314"^^xsd:anyURI .

C1901A00006:1281 a legcons:Item,
        skos:Concept,
        dcat:Resource ;
    rdfs:label "Item I1281"@en-AU ;
    rdfs:comment "261  Imprisonment not to release penalty - GraphNodeID: I1281"@en-AU ;
    skos:definition "261  Imprisonment not to release penalty"@en-AU ;
    skos:narrower C1901A00006:1162 ;
    skos:prefLabel "Item I1281"@en-AU ;
    dcat:accessURL "https://www.legislation.gov.au/C1901A00006/2024-07-01/2024-07-01/text/original/epub/OEBPS/document_3/document_3.html#_Toc172627315"^^xsd:anyURI .

C1901A00006:1282 a legcons:Item,
        skos:Concept,
        dcat:Resource ;
    rdfs:label "Item I1282"@en-AU ;
    rdfs:comment "263  Parties may recover costs - GraphNodeID: I1282"@en-AU ;
    skos:definition "263  Parties may recover costs"@en-AU ;
    skos:narrower C1901A00006:1162 ;
    skos:prefLabel "Item I1282"@en-AU ;
    dcat:accessURL "https://www.legislation.gov.au/C1901A00006/2024-07-01/2024-07-01/text/original/epub/OEBPS/document_3/document_3.html#_Toc172627316"^^xsd:anyURI .

C1901A00006:1283 a legcons:Item,
        skos:Concept,
        dcat:Resource ;
    rdfs:label "Item I1283"@en-AU ;
    rdfs:comment "264  Application of penalties - GraphNodeID: I1283"@en-AU ;
    skos:definition "264  Application of penalties"@en-AU ;
    skos:narrower C1901A00006:1162 ;
    skos:prefLabel "Item I1283"@en-AU ;
    dcat:accessURL "https://www.legislation.gov.au/C1901A00006/2024-07-01/2024-07-01/text/original/epub/OEBPS/document_3/document_3.html#_Toc172627317"^^xsd:anyURI .

C1901A00006:1284 a legcons:Part,
        skos:Concept,
        dcat:Resource ;
    rdfs:label "Part P1284"@en-AU ;
    rdfs:comment "Part XVTenders for rights to enter goods for home consumption at concessional rates - GraphNodeID: P1284"@en-AU ;
    skos:definition "Part XVTenders for rights to enter goods for home consumption at concessional rates"@en-AU ;
    skos:narrower C1901A00006:952 ;
    skos:prefLabel "Part P1284"@en-AU ;
    dcat:accessURL "https://www.legislation.gov.au/C1901A00006/2024-07-01/2024-07-01/text/original/epub/OEBPS/document_3/document_3.html#_Toc172627318"^^xsd:anyURI .

C1901A00006:1285 a legcons:Item,
        skos:Concept,
        dcat:Resource ;
    rdfs:label "Item I1285"@en-AU ;
    rdfs:comment "265  Interpretation - GraphNodeID: I1285"@en-AU ;
    skos:definition "265  Interpretation"@en-AU ;
    skos:narrower C1901A00006:1162 ;
    skos:prefLabel "Item I1285"@en-AU ;
    dcat:accessURL "https://www.legislation.gov.au/C1901A00006/2024-07-01/2024-07-01/text/original/epub/OEBPS/document_3/document_3.html#_Toc172627319"^^xsd:anyURI .

C1901A00006:1286 a legcons:Item,
        skos:Concept,
        dcat:Resource ;
    rdfs:label "Item I1286"@en-AU ;
    rdfs:comment "266  Tender schemes - GraphNodeID: I1286"@en-AU ;
    skos:definition "266  Tender schemes"@en-AU ;
    skos:narrower C1901A00006:1162 ;
    skos:prefLabel "Item I1286"@en-AU ;
    dcat:accessURL "https://www.legislation.gov.au/C1901A00006/2024-07-01/2024-07-01/text/original/epub/OEBPS/document_3/document_3.html#_Toc172627320"^^xsd:anyURI .

C1901A00006:1287 a legcons:Item,
        skos:Concept,
        dcat:Resource ;
    rdfs:label "Item I1287"@en-AU ;
    rdfs:comment "267  Undertakings relating to tenders - GraphNodeID: I1287"@en-AU ;
    skos:definition "267  Undertakings relating to tenders"@en-AU ;
    skos:narrower C1901A00006:1162 ;
    skos:prefLabel "Item I1287"@en-AU ;
    dcat:accessURL "https://www.legislation.gov.au/C1901A00006/2024-07-01/2024-07-01/text/original/epub/OEBPS/document_3/document_3.html#_Toc172627321"^^xsd:anyURI .

C1901A00006:1288 a legcons:Item,
        skos:Concept,
        dcat:Resource ;
    rdfs:label "Item I1288"@en-AU ;
    rdfs:comment "268  Transfers of rights to enter goods for home consumption at concessional rates of duty - GraphNodeID: I1288"@en-AU ;
    skos:definition "268  Transfers of rights to enter goods for home consumption at concessional rates of duty"@en-AU ;
    skos:narrower C1901A00006:1162 ;
    skos:prefLabel "Item I1288"@en-AU ;
    dcat:accessURL "https://www.legislation.gov.au/C1901A00006/2024-07-01/2024-07-01/text/original/epub/OEBPS/document_3/document_3.html#_Toc172627322"^^xsd:anyURI .

C1901A00006:1289 a legcons:Item,
        skos:Concept,
        dcat:Resource ;
    rdfs:label "Item I1289"@en-AU ;
    rdfs:comment "269  Revocation or variation of undertaking - GraphNodeID: I1289"@en-AU ;
    skos:definition "269  Revocation or variation of undertaking"@en-AU ;
    skos:narrower C1901A00006:1162 ;
    skos:prefLabel "Item I1289"@en-AU ;
    dcat:accessURL "https://www.legislation.gov.au/C1901A00006/2024-07-01/2024-07-01/text/original/epub/OEBPS/document_3/document_3.html#_Toc172627323"^^xsd:anyURI .

C1901A00006:129 a legcons:Item,
        skos:Concept,
        dcat:Resource ;
    rdfs:label "Item I129"@en-AU ;
    rdfs:comment "71 AAAB  Report and grant of authority to deal with Subdivision AA goods - GraphNodeID: I129"@en-AU ;
    skos:definition "71 AAAB  Report and grant of authority to deal with Subdivision AA goods"@en-AU ;
    skos:narrower C1901A00006:127 ;
    skos:prefLabel "Item I129"@en-AU ;
    dcat:accessURL "https://www.legislation.gov.au/C1901A00006/2024-07-01/2024-07-01/text/original/epub/OEBPS/document_1/document_1.html#_Toc172623103"^^xsd:anyURI .

C1901A00006:1290 a legcons:Item,
        skos:Concept,
        dcat:Resource ;
    rdfs:label "Item I1290"@en-AU ;
    rdfs:comment "269 A  Recovery of penalties - GraphNodeID: I1290"@en-AU ;
    skos:definition "269 A  Recovery of penalties"@en-AU ;
    skos:narrower C1901A00006:1162 ;
    skos:prefLabel "Item I1290"@en-AU ;
    dcat:accessURL "https://www.legislation.gov.au/C1901A00006/2024-07-01/2024-07-01/text/original/epub/OEBPS/document_3/document_3.html#_Toc172627324"^^xsd:anyURI .

C1901A00006:1292 a legcons:Division,
        skos:Concept,
        dcat:Resource ;
    rdfs:label "Division D1292"@en-AU ;
    rdfs:comment "Division 1 Preliminary - GraphNodeID: D1292"@en-AU ;
    skos:definition "Division 1 Preliminary"@en-AU ;
    skos:narrower C1901A00006:1291 ;
    skos:prefLabel "Division D1292"@en-AU ;
    dcat:accessURL "https://www.legislation.gov.au/C1901A00006/2024-07-01/2024-07-01/text/original/epub/OEBPS/document_3/document_3.html#_Toc172627326"^^xsd:anyURI .

C1901A00006:1293 a legcons:Item,
        skos:Concept,
        dcat:Resource ;
    rdfs:label "Item I1293"@en-AU ;
    rdfs:comment "269 B  Interpretation - GraphNodeID: I1293"@en-AU ;
    skos:definition "269 B  Interpretation"@en-AU ;
    skos:narrower C1901A00006:1162 ;
    skos:prefLabel "Item I1293"@en-AU ;
    dcat:accessURL "https://www.legislation.gov.au/C1901A00006/2024-07-01/2024-07-01/text/original/epub/OEBPS/document_3/document_3.html#_Toc172627327"^^xsd:anyURI .

C1901A00006:1294 a legcons:Item,
        skos:Concept,
        dcat:Resource ;
    rdfs:label "Item I1294"@en-AU ;
    rdfs:comment "269 C  Interpretationcore criteria - GraphNodeID: I1294"@en-AU ;
    skos:definition "269 C  Interpretationcore criteria"@en-AU ;
    skos:narrower C1901A00006:1162 ;
    skos:prefLabel "Item I1294"@en-AU ;
    dcat:accessURL "https://www.legislation.gov.au/C1901A00006/2024-07-01/2024-07-01/text/original/epub/OEBPS/document_3/document_3.html#_Toc172627328"^^xsd:anyURI .

C1901A00006:1295 a legcons:Item,
        skos:Concept,
        dcat:Resource ;
    rdfs:label "Item I1295"@en-AU ;
    rdfs:comment "269 D  Interpretationgoods produced in Australia - GraphNodeID: I1295"@en-AU ;
    skos:definition "269 D  Interpretationgoods produced in Australia"@en-AU ;
    skos:narrower C1901A00006:1162 ;
    skos:prefLabel "Item I1295"@en-AU ;
    dcat:accessURL "https://www.legislation.gov.au/C1901A00006/2024-07-01/2024-07-01/text/original/epub/OEBPS/document_3/document_3.html#_Toc172627329"^^xsd:anyURI .

C1901A00006:1296 a legcons:Item,
        skos:Concept,
        dcat:Resource ;
    rdfs:label "Item I1296"@en-AU ;
    rdfs:comment "269 E  Interpretationthe ordinary course of business - GraphNodeID: I1296"@en-AU ;
    skos:definition "269 E  Interpretationthe ordinary course of business"@en-AU ;
    skos:narrower C1901A00006:1162 ;
    skos:prefLabel "Item I1296"@en-AU ;
    dcat:accessURL "https://www.legislation.gov.au/C1901A00006/2024-07-01/2024-07-01/text/original/epub/OEBPS/document_3/document_3.html#_Toc172627330"^^xsd:anyURI .

C1901A00006:1297 a legcons:Division,
        skos:Concept,
        dcat:Resource ;
    rdfs:label "Division D1297"@en-AU ;
    rdfs:comment "Division 2 Making and processing TCO applications - GraphNodeID: D1297"@en-AU ;
    skos:definition "Division 2 Making and processing TCO applications"@en-AU ;
    skos:narrower C1901A00006:1291 ;
    skos:prefLabel "Division D1297"@en-AU ;
    dcat:accessURL "https://www.legislation.gov.au/C1901A00006/2024-07-01/2024-07-01/text/original/epub/OEBPS/document_3/document_3.html#_Toc172627331"^^xsd:anyURI .

C1901A00006:1298 a legcons:Item,
        skos:Concept,
        dcat:Resource ;
    rdfs:label "Item I1298"@en-AU ;
    rdfs:comment "269 F  Making a TCO application - GraphNodeID: I1298"@en-AU ;
    skos:definition "269 F  Making a TCO application"@en-AU ;
    skos:narrower C1901A00006:1162 ;
    skos:prefLabel "Item I1298"@en-AU ;
    dcat:accessURL "https://www.legislation.gov.au/C1901A00006/2024-07-01/2024-07-01/text/original/epub/OEBPS/document_3/document_3.html#_Toc172627332"^^xsd:anyURI .

C1901A00006:1299 a legcons:Item,
        skos:Concept,
        dcat:Resource ;
    rdfs:label "Item I1299"@en-AU ;
    rdfs:comment "269 FA  The applicants obligation - GraphNodeID: I1299"@en-AU ;
    skos:definition "269 FA  The applicants obligation"@en-AU ;
    skos:narrower C1901A00006:1162 ;
    skos:prefLabel "Item I1299"@en-AU ;
    dcat:accessURL "https://www.legislation.gov.au/C1901A00006/2024-07-01/2024-07-01/text/original/epub/OEBPS/document_3/document_3.html#_Toc172627333"^^xsd:anyURI .

C1901A00006:13 a legcons:Item,
        skos:Concept,
        dcat:Resource ;
    rdfs:label "Item I13"@en-AU ;
    rdfs:comment "5 AA  Application of the Criminal Code - GraphNodeID: I13"@en-AU ;
    skos:definition "5 AA  Application of the Criminal Code"@en-AU ;
    skos:narrower C1901A00006:2 ;
    skos:prefLabel "Item I13"@en-AU ;
    dcat:accessURL "https://www.legislation.gov.au/C1901A00006/2024-07-01/2024-07-01/text/original/epub/OEBPS/document_1/document_1.html#_Toc172622987"^^xsd:anyURI .

C1901A00006:130 a legcons:Item,
        skos:Concept,
        dcat:Resource ;
    rdfs:label "Item I130"@en-AU ;
    rdfs:comment "71 AAAC  Suspension of authority to deal with Subdivision AA goods - GraphNodeID: I130"@en-AU ;
    skos:definition "71 AAAC  Suspension of authority to deal with Subdivision AA goods"@en-AU ;
    skos:narrower C1901A00006:127 ;
    skos:prefLabel "Item I130"@en-AU ;
    dcat:accessURL "https://www.legislation.gov.au/C1901A00006/2024-07-01/2024-07-01/text/original/epub/OEBPS/document_1/document_1.html#_Toc172623104"^^xsd:anyURI .

C1901A00006:1300 a legcons:Item,
        skos:Concept,
        dcat:Resource ;
    rdfs:label "Item I1300"@en-AU ;
    rdfs:comment "269 G  Withdrawing a TCO application - GraphNodeID: I1300"@en-AU ;
    skos:definition "269 G  Withdrawing a TCO application"@en-AU ;
    skos:narrower C1901A00006:1162 ;
    skos:prefLabel "Item I1300"@en-AU ;
    dcat:accessURL "https://www.legislation.gov.au/C1901A00006/2024-07-01/2024-07-01/text/original/epub/OEBPS/document_3/document_3.html#_Toc172627334"^^xsd:anyURI .

C1901A00006:1301 a legcons:Item,
        skos:Concept,
        dcat:Resource ;
    rdfs:label "Item I1301"@en-AU ;
    rdfs:comment "269 H  Screening the application - GraphNodeID: I1301"@en-AU ;
    skos:definition "269 H  Screening the application"@en-AU ;
    skos:narrower C1901A00006:1162 ;
    skos:prefLabel "Item I1301"@en-AU ;
    dcat:accessURL "https://www.legislation.gov.au/C1901A00006/2024-07-01/2024-07-01/text/original/epub/OEBPS/document_3/document_3.html#_Toc172627335"^^xsd:anyURI .

C1901A00006:1302 a legcons:Item,
        skos:Concept,
        dcat:Resource ;
    rdfs:label "Item I1302"@en-AU ;
    rdfs:comment "269 HA  Comptroller General of Customs may reject a TCO application in relation to goods referred to in section 269 SJ - GraphNodeID: I1302"@en-AU ;
    skos:definition "269 HA  Comptroller General of Customs may reject a TCO application in relation to goods referred to in section 269 SJ"@en-AU ;
    skos:narrower C1901A00006:1162 ;
    skos:prefLabel "Item I1302"@en-AU ;
    dcat:accessURL "https://www.legislation.gov.au/C1901A00006/2024-07-01/2024-07-01/text/original/epub/OEBPS/document_3/document_3.html#_Toc172627336"^^xsd:anyURI .

C1901A00006:1303 a legcons:Item,
        skos:Concept,
        dcat:Resource ;
    rdfs:label "Item I1303"@en-AU ;
    rdfs:comment "269 J  Applications taken to be lodged in certain circumstances - GraphNodeID: I1303"@en-AU ;
    skos:definition "269 J  Applications taken to be lodged in certain circumstances"@en-AU ;
    skos:narrower C1901A00006:1162 ;
    skos:prefLabel "Item I1303"@en-AU ;
    dcat:accessURL "https://www.legislation.gov.au/C1901A00006/2024-07-01/2024-07-01/text/original/epub/OEBPS/document_3/document_3.html#_Toc172627337"^^xsd:anyURI .

C1901A00006:1304 a legcons:Item,
        skos:Concept,
        dcat:Resource ;
    rdfs:label "Item I1304"@en-AU ;
    rdfs:comment "269 K  Processing a valid application - GraphNodeID: I1304"@en-AU ;
    skos:definition "269 K  Processing a valid application"@en-AU ;
    skos:narrower C1901A00006:1162 ;
    skos:prefLabel "Item I1304"@en-AU ;
    dcat:accessURL "https://www.legislation.gov.au/C1901A00006/2024-07-01/2024-07-01/text/original/epub/OEBPS/document_3/document_3.html#_Toc172627338"^^xsd:anyURI .

C1901A00006:1305 a legcons:Item,
        skos:Concept,
        dcat:Resource ;
    rdfs:label "Item I1305"@en-AU ;
    rdfs:comment "269 L  Amendment of TCO applications - GraphNodeID: I1305"@en-AU ;
    skos:definition "269 L  Amendment of TCO applications"@en-AU ;
    skos:narrower C1901A00006:1162 ;
    skos:prefLabel "Item I1305"@en-AU ;
    dcat:accessURL "https://www.legislation.gov.au/C1901A00006/2024-07-01/2024-07-01/text/original/epub/OEBPS/document_3/document_3.html#_Toc172627339"^^xsd:anyURI .

C1901A00006:1306 a legcons:Item,
        skos:Concept,
        dcat:Resource ;
    rdfs:label "Item I1306"@en-AU ;
    rdfs:comment "269 M  Comptroller General of Customs may invite submissions or seek other information documents or material - GraphNodeID: I1306"@en-AU ;
    skos:definition "269 M  Comptroller General of Customs may invite submissions or seek other information documents or material"@en-AU ;
    skos:narrower C1901A00006:1162 ;
    skos:prefLabel "Item I1306"@en-AU ;
    dcat:accessURL "https://www.legislation.gov.au/C1901A00006/2024-07-01/2024-07-01/text/original/epub/OEBPS/document_3/document_3.html#_Toc172627340"^^xsd:anyURI .

C1901A00006:1307 a legcons:Item,
        skos:Concept,
        dcat:Resource ;
    rdfs:label "Item I1307"@en-AU ;
    rdfs:comment "269 N  Reprocessing of TCO applications - GraphNodeID: I1307"@en-AU ;
    skos:definition "269 N  Reprocessing of TCO applications"@en-AU ;
    skos:narrower C1901A00006:1162 ;
    skos:prefLabel "Item I1307"@en-AU ;
    dcat:accessURL "https://www.legislation.gov.au/C1901A00006/2024-07-01/2024-07-01/text/original/epub/OEBPS/document_3/document_3.html#_Toc172627341"^^xsd:anyURI .

C1901A00006:1308 a legcons:Division,
        skos:Concept,
        dcat:Resource ;
    rdfs:label "Division D1308"@en-AU ;
    rdfs:comment "Division 3 Making and operation of TCOs - GraphNodeID: D1308"@en-AU ;
    skos:definition "Division 3 Making and operation of TCOs"@en-AU ;
    skos:narrower C1901A00006:1291 ;
    skos:prefLabel "Division D1308"@en-AU ;
    dcat:accessURL "https://www.legislation.gov.au/C1901A00006/2024-07-01/2024-07-01/text/original/epub/OEBPS/document_3/document_3.html#_Toc172627342"^^xsd:anyURI .

C1901A00006:1309 a legcons:Item,
        skos:Concept,
        dcat:Resource ;
    rdfs:label "Item I1309"@en-AU ;
    rdfs:comment "269 P  The making of a standard TCO - GraphNodeID: I1309"@en-AU ;
    skos:definition "269 P  The making of a standard TCO"@en-AU ;
    skos:narrower C1901A00006:1162 ;
    skos:prefLabel "Item I1309"@en-AU ;
    dcat:accessURL "https://www.legislation.gov.au/C1901A00006/2024-07-01/2024-07-01/text/original/epub/OEBPS/document_3/document_3.html#_Toc172627343"^^xsd:anyURI .

C1901A00006:1310 a legcons:Item,
        skos:Concept,
        dcat:Resource ;
    rdfs:label "Item I1310"@en-AU ;
    rdfs:comment "269 Q  The making of a TCO for goods requiring repair - GraphNodeID: I1310"@en-AU ;
    skos:definition "269 Q  The making of a TCO for goods requiring repair"@en-AU ;
    skos:narrower C1901A00006:1162 ;
    skos:prefLabel "Item I1310"@en-AU ;
    dcat:accessURL "https://www.legislation.gov.au/C1901A00006/2024-07-01/2024-07-01/text/original/epub/OEBPS/document_3/document_3.html#_Toc172627344"^^xsd:anyURI .

C1901A00006:1311 a legcons:Item,
        skos:Concept,
        dcat:Resource ;
    rdfs:label "Item I1311"@en-AU ;
    rdfs:comment "269 R  Notification of TCO decisions - GraphNodeID: I1311"@en-AU ;
    skos:definition "269 R  Notification of TCO decisions"@en-AU ;
    skos:narrower C1901A00006:1162 ;
    skos:prefLabel "Item I1311"@en-AU ;
    dcat:accessURL "https://www.legislation.gov.au/C1901A00006/2024-07-01/2024-07-01/text/original/epub/OEBPS/document_3/document_3.html#_Toc172627345"^^xsd:anyURI .

C1901A00006:1312 a legcons:Item,
        skos:Concept,
        dcat:Resource ;
    rdfs:label "Item I1312"@en-AU ;
    rdfs:comment "269 S  Operation of TCOs - GraphNodeID: I1312"@en-AU ;
    skos:definition "269 S  Operation of TCOs"@en-AU ;
    skos:narrower C1901A00006:1162 ;
    skos:prefLabel "Item I1312"@en-AU ;
    dcat:accessURL "https://www.legislation.gov.au/C1901A00006/2024-07-01/2024-07-01/text/original/epub/OEBPS/document_3/document_3.html#_Toc172627346"^^xsd:anyURI .

C1901A00006:1313 a legcons:Item,
        skos:Concept,
        dcat:Resource ;
    rdfs:label "Item I1313"@en-AU ;
    rdfs:comment "269 SA  Consequence of commencement or cessation of production before TCO decision - GraphNodeID: I1313"@en-AU ;
    skos:definition "269 SA  Consequence of commencement or cessation of production before TCO decision"@en-AU ;
    skos:narrower C1901A00006:1162 ;
    skos:prefLabel "Item I1313"@en-AU ;
    dcat:accessURL "https://www.legislation.gov.au/C1901A00006/2024-07-01/2024-07-01/text/original/epub/OEBPS/document_3/document_3.html#_Toc172627347"^^xsd:anyURI .

C1901A00006:1314 a legcons:Division,
        skos:Concept,
        dcat:Resource ;
    rdfs:label "Division D1314"@en-AU ;
    rdfs:comment "Division 4 Revocation of TCOs - GraphNodeID: D1314"@en-AU ;
    skos:definition "Division 4 Revocation of TCOs"@en-AU ;
    skos:narrower C1901A00006:1291 ;
    skos:prefLabel "Division D1314"@en-AU ;
    dcat:accessURL "https://www.legislation.gov.au/C1901A00006/2024-07-01/2024-07-01/text/original/epub/OEBPS/document_3/document_3.html#_Toc172627348"^^xsd:anyURI .

C1901A00006:1315 a legcons:Item,
        skos:Concept,
        dcat:Resource ;
    rdfs:label "Item I1315"@en-AU ;
    rdfs:comment "269 SB  Request for revocation of TCOs - GraphNodeID: I1315"@en-AU ;
    skos:definition "269 SB  Request for revocation of TCOs"@en-AU ;
    skos:narrower C1901A00006:1162 ;
    skos:prefLabel "Item I1315"@en-AU ;
    dcat:accessURL "https://www.legislation.gov.au/C1901A00006/2024-07-01/2024-07-01/text/original/epub/OEBPS/document_3/document_3.html#_Toc172627349"^^xsd:anyURI .

C1901A00006:1316 a legcons:Item,
        skos:Concept,
        dcat:Resource ;
    rdfs:label "Item I1316"@en-AU ;
    rdfs:comment "269 SC  Processing requests for revocation of TCOs - GraphNodeID: I1316"@en-AU ;
    skos:definition "269 SC  Processing requests for revocation of TCOs"@en-AU ;
    skos:narrower C1901A00006:1162 ;
    skos:prefLabel "Item I1316"@en-AU ;
    dcat:accessURL "https://www.legislation.gov.au/C1901A00006/2024-07-01/2024-07-01/text/original/epub/OEBPS/document_3/document_3.html#_Toc172627350"^^xsd:anyURI .

C1901A00006:1317 a legcons:Item,
        skos:Concept,
        dcat:Resource ;
    rdfs:label "Item I1317"@en-AU ;
    rdfs:comment "269 SD  Revocation at the initiative of Comptroller General of Customs - GraphNodeID: I1317"@en-AU ;
    skos:definition "269 SD  Revocation at the initiative of Comptroller General of Customs"@en-AU ;
    skos:narrower C1901A00006:1162 ;
    skos:prefLabel "Item I1317"@en-AU ;
    dcat:accessURL "https://www.legislation.gov.au/C1901A00006/2024-07-01/2024-07-01/text/original/epub/OEBPS/document_3/document_3.html#_Toc172627351"^^xsd:anyURI .

C1901A00006:1318 a legcons:Item,
        skos:Concept,
        dcat:Resource ;
    rdfs:label "Item I1318"@en-AU ;
    rdfs:comment "269 SE  Notification of revocation decisions - GraphNodeID: I1318"@en-AU ;
    skos:definition "269 SE  Notification of revocation decisions"@en-AU ;
    skos:narrower C1901A00006:1162 ;
    skos:prefLabel "Item I1318"@en-AU ;
    dcat:accessURL "https://www.legislation.gov.au/C1901A00006/2024-07-01/2024-07-01/text/original/epub/OEBPS/document_3/document_3.html#_Toc172627352"^^xsd:anyURI .

C1901A00006:1319 a legcons:Item,
        skos:Concept,
        dcat:Resource ;
    rdfs:label "Item I1319"@en-AU ;
    rdfs:comment "269 SF  Comptroller General of Customs may seek information documents or material relating to revocation - GraphNodeID: I1319"@en-AU ;
    skos:definition "269 SF  Comptroller General of Customs may seek information documents or material relating to revocation"@en-AU ;
    skos:narrower C1901A00006:1162 ;
    skos:prefLabel "Item I1319"@en-AU ;
    dcat:accessURL "https://www.legislation.gov.au/C1901A00006/2024-07-01/2024-07-01/text/original/epub/OEBPS/document_3/document_3.html#_Toc172627353"^^xsd:anyURI .

C1901A00006:132 a legcons:Item,
        skos:Concept,
        dcat:Resource ;
    rdfs:label "Item I132"@en-AU ;
    rdfs:comment "71 AAAD  Meaning of specified low value goods - GraphNodeID: I132"@en-AU ;
    skos:definition "71 AAAD  Meaning of specified low value goods"@en-AU ;
    skos:narrower C1901A00006:131 ;
    skos:prefLabel "Item I132"@en-AU ;
    dcat:accessURL "https://www.legislation.gov.au/C1901A00006/2024-07-01/2024-07-01/text/original/epub/OEBPS/document_1/document_1.html#_Toc172623106"^^xsd:anyURI .

C1901A00006:1320 a legcons:Item,
        skos:Concept,
        dcat:Resource ;
    rdfs:label "Item I1320"@en-AU ;
    rdfs:comment "269 SG  Effect of revocation on goods in transit and capital equipment on order - GraphNodeID: I1320"@en-AU ;
    skos:definition "269 SG  Effect of revocation on goods in transit and capital equipment on order"@en-AU ;
    skos:narrower C1901A00006:1162 ;
    skos:prefLabel "Item I1320"@en-AU ;
    dcat:accessURL "https://www.legislation.gov.au/C1901A00006/2024-07-01/2024-07-01/text/original/epub/OEBPS/document_3/document_3.html#_Toc172627354"^^xsd:anyURI .

C1901A00006:1321 a legcons:Division,
        skos:Concept,
        dcat:Resource ;
    rdfs:label "Division D1321"@en-AU ;
    rdfs:comment "Division 5 Miscellaneous - GraphNodeID: D1321"@en-AU ;
    skos:definition "Division 5 Miscellaneous"@en-AU ;
    skos:narrower C1901A00006:1291 ;
    skos:prefLabel "Division D1321"@en-AU ;
    dcat:accessURL "https://www.legislation.gov.au/C1901A00006/2024-07-01/2024-07-01/text/original/epub/OEBPS/document_3/document_3.html#_Toc172627355"^^xsd:anyURI .

C1901A00006:1322 a legcons:Item,
        skos:Concept,
        dcat:Resource ;
    rdfs:label "Item I1322"@en-AU ;
    rdfs:comment "269 SH  Internal review - GraphNodeID: I1322"@en-AU ;
    skos:definition "269 SH  Internal review"@en-AU ;
    skos:narrower C1901A00006:1162 ;
    skos:prefLabel "Item I1322"@en-AU ;
    dcat:accessURL "https://www.legislation.gov.au/C1901A00006/2024-07-01/2024-07-01/text/original/epub/OEBPS/document_3/document_3.html#_Toc172627356"^^xsd:anyURI .

C1901A00006:1323 a legcons:Item,
        skos:Concept,
        dcat:Resource ;
    rdfs:label "Item I1323"@en-AU ;
    rdfs:comment "269 SHA  Administrative Appeals Tribunal Review of reconsideration decisions - GraphNodeID: I1323"@en-AU ;
    skos:definition "269 SHA  Administrative Appeals Tribunal Review of reconsideration decisions"@en-AU ;
    skos:narrower C1901A00006:1162 ;
    skos:prefLabel "Item I1323"@en-AU ;
    dcat:accessURL "https://www.legislation.gov.au/C1901A00006/2024-07-01/2024-07-01/text/original/epub/OEBPS/document_3/document_3.html#_Toc172627357"^^xsd:anyURI .

C1901A00006:1324 a legcons:Item,
        skos:Concept,
        dcat:Resource ;
    rdfs:label "Item I1324"@en-AU ;
    rdfs:comment "269 SJ  TCOs not to apply to goods described by reference to their end use or certain goods - GraphNodeID: I1324"@en-AU ;
    skos:definition "269 SJ  TCOs not to apply to goods described by reference to their end use or certain goods"@en-AU ;
    skos:narrower C1901A00006:1162 ;
    skos:prefLabel "Item I1324"@en-AU ;
    dcat:accessURL "https://www.legislation.gov.au/C1901A00006/2024-07-01/2024-07-01/text/original/epub/OEBPS/document_3/document_3.html#_Toc172627358"^^xsd:anyURI .

C1901A00006:1325 a legcons:Item,
        skos:Concept,
        dcat:Resource ;
    rdfs:label "Item I1325"@en-AU ;
    rdfs:comment "269 SK  TCOs not to contravene international agreements - GraphNodeID: I1325"@en-AU ;
    skos:definition "269 SK  TCOs not to contravene international agreements"@en-AU ;
    skos:narrower C1901A00006:1162 ;
    skos:prefLabel "Item I1325"@en-AU ;
    dcat:accessURL "https://www.legislation.gov.au/C1901A00006/2024-07-01/2024-07-01/text/original/epub/OEBPS/document_3/document_3.html#_Toc172627359"^^xsd:anyURI .

C1901A00006:1328 a legcons:Item,
        skos:Concept,
        dcat:Resource ;
    rdfs:label "Item I1328"@en-AU ;
    rdfs:comment "269 SM  Overview of Part - GraphNodeID: I1328"@en-AU ;
    skos:definition "269 SM  Overview of Part"@en-AU ;
    skos:narrower C1901A00006:1162 ;
    skos:prefLabel "Item I1328"@en-AU ;
    dcat:accessURL "https://www.legislation.gov.au/C1901A00006/2024-07-01/2024-07-01/text/original/epub/OEBPS/document_4/document_4.html#_Toc172628762"^^xsd:anyURI .

C1901A00006:133 a legcons:Item,
        skos:Concept,
        dcat:Resource ;
    rdfs:label "Item I133"@en-AU ;
    rdfs:comment "71 AAAE  Regulations - GraphNodeID: I133"@en-AU ;
    skos:definition "71 AAAE  Regulations"@en-AU ;
    skos:narrower C1901A00006:131 ;
    skos:prefLabel "Item I133"@en-AU ;
    dcat:accessURL "https://www.legislation.gov.au/C1901A00006/2024-07-01/2024-07-01/text/original/epub/OEBPS/document_1/document_1.html#_Toc172623107"^^xsd:anyURI .

C1901A00006:1331 a legcons:Item,
        skos:Concept,
        dcat:Resource ;
    rdfs:label "Item I1331"@en-AU ;
    rdfs:comment "269 SMA  What this Division is about - GraphNodeID: I1331"@en-AU ;
    skos:definition "269 SMA  What this Division is about"@en-AU ;
    skos:narrower C1901A00006:1330 ;
    skos:prefLabel "Item I1331"@en-AU ;
    dcat:accessURL "https://www.legislation.gov.au/C1901A00006/2024-07-01/2024-07-01/text/original/epub/OEBPS/document_4/document_4.html#_Toc172628765"^^xsd:anyURI .

C1901A00006:1333 a legcons:Item,
        skos:Concept,
        dcat:Resource ;
    rdfs:label "Item I1333"@en-AU ;
    rdfs:comment "269 SMB  Establishment - GraphNodeID: I1333"@en-AU ;
    skos:definition "269 SMB  Establishment"@en-AU ;
    skos:narrower C1901A00006:1332 ;
    skos:prefLabel "Item I1333"@en-AU ;
    dcat:accessURL "https://www.legislation.gov.au/C1901A00006/2024-07-01/2024-07-01/text/original/epub/OEBPS/document_4/document_4.html#_Toc172628767"^^xsd:anyURI .

C1901A00006:1334 a legcons:Item,
        skos:Concept,
        dcat:Resource ;
    rdfs:label "Item I1334"@en-AU ;
    rdfs:comment "269 SMC  Constitution of the Anti Dumping Commission - GraphNodeID: I1334"@en-AU ;
    skos:definition "269 SMC  Constitution of the Anti Dumping Commission"@en-AU ;
    skos:narrower C1901A00006:1332 ;
    skos:prefLabel "Item I1334"@en-AU ;
    dcat:accessURL "https://www.legislation.gov.au/C1901A00006/2024-07-01/2024-07-01/text/original/epub/OEBPS/document_4/document_4.html#_Toc172628768"^^xsd:anyURI .

C1901A00006:1335 a legcons:Item,
        skos:Concept,
        dcat:Resource ;
    rdfs:label "Item I1335"@en-AU ;
    rdfs:comment "269 SMD  Function of the Anti Dumping Commission - GraphNodeID: I1335"@en-AU ;
    skos:definition "269 SMD  Function of the Anti Dumping Commission"@en-AU ;
    skos:narrower C1901A00006:1332 ;
    skos:prefLabel "Item I1335"@en-AU ;
    dcat:accessURL "https://www.legislation.gov.au/C1901A00006/2024-07-01/2024-07-01/text/original/epub/OEBPS/document_4/document_4.html#_Toc172628769"^^xsd:anyURI .

C1901A00006:1336 a legcons:Item,
        skos:Concept,
        dcat:Resource ;
    rdfs:label "Item I1336"@en-AU ;
    rdfs:comment "269 SME  Anti Dumping Commission has privileges and immunities of the Crown - GraphNodeID: I1336"@en-AU ;
    skos:definition "269 SME  Anti Dumping Commission has privileges and immunities of the Crown"@en-AU ;
    skos:narrower C1901A00006:1332 ;
    skos:prefLabel "Item I1336"@en-AU ;
    dcat:accessURL "https://www.legislation.gov.au/C1901A00006/2024-07-01/2024-07-01/text/original/epub/OEBPS/document_4/document_4.html#_Toc172628770"^^xsd:anyURI .

C1901A00006:1338 a legcons:Item,
        skos:Concept,
        dcat:Resource ;
    rdfs:label "Item I1338"@en-AU ;
    rdfs:comment "269 SMF  Establishment - GraphNodeID: I1338"@en-AU ;
    skos:definition "269 SMF  Establishment"@en-AU ;
    skos:narrower C1901A00006:1337 ;
    skos:prefLabel "Item I1338"@en-AU ;
    dcat:accessURL "https://www.legislation.gov.au/C1901A00006/2024-07-01/2024-07-01/text/original/epub/OEBPS/document_4/document_4.html#_Toc172628772"^^xsd:anyURI .

C1901A00006:1339 a legcons:Item,
        skos:Concept,
        dcat:Resource ;
    rdfs:label "Item I1339"@en-AU ;
    rdfs:comment "269 SMG  Powers of Commissioner - GraphNodeID: I1339"@en-AU ;
    skos:definition "269 SMG  Powers of Commissioner"@en-AU ;
    skos:narrower C1901A00006:1337 ;
    skos:prefLabel "Item I1339"@en-AU ;
    dcat:accessURL "https://www.legislation.gov.au/C1901A00006/2024-07-01/2024-07-01/text/original/epub/OEBPS/document_4/document_4.html#_Toc172628773"^^xsd:anyURI .

C1901A00006:134 a legcons:Item,
        skos:Concept,
        dcat:Resource ;
    rdfs:label "Item I134"@en-AU ;
    rdfs:comment "71 AAAF  Making a self assessed clearance declaration - GraphNodeID: I134"@en-AU ;
    skos:definition "71 AAAF  Making a self assessed clearance declaration"@en-AU ;
    skos:narrower C1901A00006:131 ;
    skos:prefLabel "Item I134"@en-AU ;
    dcat:accessURL "https://www.legislation.gov.au/C1901A00006/2024-07-01/2024-07-01/text/original/epub/OEBPS/document_1/document_1.html#_Toc172623108"^^xsd:anyURI .

C1901A00006:1340 a legcons:Item,
        skos:Concept,
        dcat:Resource ;
    rdfs:label "Item I1340"@en-AU ;
    rdfs:comment "269 SMH  Appointment - GraphNodeID: I1340"@en-AU ;
    skos:definition "269 SMH  Appointment"@en-AU ;
    skos:narrower C1901A00006:1337 ;
    skos:prefLabel "Item I1340"@en-AU ;
    dcat:accessURL "https://www.legislation.gov.au/C1901A00006/2024-07-01/2024-07-01/text/original/epub/OEBPS/document_4/document_4.html#_Toc172628774"^^xsd:anyURI .

C1901A00006:1341 a legcons:Item,
        skos:Concept,
        dcat:Resource ;
    rdfs:label "Item I1341"@en-AU ;
    rdfs:comment "269 SMI  Term of appointment - GraphNodeID: I1341"@en-AU ;
    skos:definition "269 SMI  Term of appointment"@en-AU ;
    skos:narrower C1901A00006:1337 ;
    skos:prefLabel "Item I1341"@en-AU ;
    dcat:accessURL "https://www.legislation.gov.au/C1901A00006/2024-07-01/2024-07-01/text/original/epub/OEBPS/document_4/document_4.html#_Toc172628775"^^xsd:anyURI .

C1901A00006:1342 a legcons:Item,
        skos:Concept,
        dcat:Resource ;
    rdfs:label "Item I1342"@en-AU ;
    rdfs:comment "269 SMJ  Acting Commissioner - GraphNodeID: I1342"@en-AU ;
    skos:definition "269 SMJ  Acting Commissioner"@en-AU ;
    skos:narrower C1901A00006:1337 ;
    skos:prefLabel "Item I1342"@en-AU ;
    dcat:accessURL "https://www.legislation.gov.au/C1901A00006/2024-07-01/2024-07-01/text/original/epub/OEBPS/document_4/document_4.html#_Toc172628776"^^xsd:anyURI .

C1901A00006:1343 a legcons:Item,
        skos:Concept,
        dcat:Resource ;
    rdfs:label "Item I1343"@en-AU ;
    rdfs:comment "269 SMK  Terms and conditions of appointment - GraphNodeID: I1343"@en-AU ;
    skos:definition "269 SMK  Terms and conditions of appointment"@en-AU ;
    skos:narrower C1901A00006:1337 ;
    skos:prefLabel "Item I1343"@en-AU ;
    dcat:accessURL "https://www.legislation.gov.au/C1901A00006/2024-07-01/2024-07-01/text/original/epub/OEBPS/document_4/document_4.html#_Toc172628777"^^xsd:anyURI .

C1901A00006:1344 a legcons:Item,
        skos:Concept,
        dcat:Resource ;
    rdfs:label "Item I1344"@en-AU ;
    rdfs:comment "269 SML  Disclosure of interests - GraphNodeID: I1344"@en-AU ;
    skos:definition "269 SML  Disclosure of interests"@en-AU ;
    skos:narrower C1901A00006:1337 ;
    skos:prefLabel "Item I1344"@en-AU ;
    dcat:accessURL "https://www.legislation.gov.au/C1901A00006/2024-07-01/2024-07-01/text/original/epub/OEBPS/document_4/document_4.html#_Toc172628778"^^xsd:anyURI .

C1901A00006:1345 a legcons:Item,
        skos:Concept,
        dcat:Resource ;
    rdfs:label "Item I1345"@en-AU ;
    rdfs:comment "269 SMM  Outside employment - GraphNodeID: I1345"@en-AU ;
    skos:definition "269 SMM  Outside employment"@en-AU ;
    skos:narrower C1901A00006:1337 ;
    skos:prefLabel "Item I1345"@en-AU ;
    dcat:accessURL "https://www.legislation.gov.au/C1901A00006/2024-07-01/2024-07-01/text/original/epub/OEBPS/document_4/document_4.html#_Toc172628779"^^xsd:anyURI .

C1901A00006:1346 a legcons:Item,
        skos:Concept,
        dcat:Resource ;
    rdfs:label "Item I1346"@en-AU ;
    rdfs:comment "269 SMN  Resignation - GraphNodeID: I1346"@en-AU ;
    skos:definition "269 SMN  Resignation"@en-AU ;
    skos:narrower C1901A00006:1337 ;
    skos:prefLabel "Item I1346"@en-AU ;
    dcat:accessURL "https://www.legislation.gov.au/C1901A00006/2024-07-01/2024-07-01/text/original/epub/OEBPS/document_4/document_4.html#_Toc172628780"^^xsd:anyURI .

C1901A00006:1347 a legcons:Item,
        skos:Concept,
        dcat:Resource ;
    rdfs:label "Item I1347"@en-AU ;
    rdfs:comment "269 SMO  Termination of appointment - GraphNodeID: I1347"@en-AU ;
    skos:definition "269 SMO  Termination of appointment"@en-AU ;
    skos:narrower C1901A00006:1337 ;
    skos:prefLabel "Item I1347"@en-AU ;
    dcat:accessURL "https://www.legislation.gov.au/C1901A00006/2024-07-01/2024-07-01/text/original/epub/OEBPS/document_4/document_4.html#_Toc172628781"^^xsd:anyURI .

C1901A00006:1349 a legcons:Item,
        skos:Concept,
        dcat:Resource ;
    rdfs:label "Item I1349"@en-AU ;
    rdfs:comment "269 SMQ  Staff - GraphNodeID: I1349"@en-AU ;
    skos:definition "269 SMQ  Staff"@en-AU ;
    skos:narrower C1901A00006:1348 ;
    skos:prefLabel "Item I1349"@en-AU ;
    dcat:accessURL "https://www.legislation.gov.au/C1901A00006/2024-07-01/2024-07-01/text/original/epub/OEBPS/document_4/document_4.html#_Toc172628783"^^xsd:anyURI .

C1901A00006:135 a legcons:Item,
        skos:Concept,
        dcat:Resource ;
    rdfs:label "Item I135"@en-AU ;
    rdfs:comment "71 AAAG  Collectors response if a self assessed clearance declaration is communicated separately from a cargo report - GraphNodeID: I135"@en-AU ;
    skos:definition "71 AAAG  Collectors response if a self assessed clearance declaration is communicated separately from a cargo report"@en-AU ;
    skos:narrower C1901A00006:131 ;
    skos:prefLabel "Item I135"@en-AU ;
    dcat:accessURL "https://www.legislation.gov.au/C1901A00006/2024-07-01/2024-07-01/text/original/epub/OEBPS/document_1/document_1.html#_Toc172623109"^^xsd:anyURI .

C1901A00006:1351 a legcons:Item,
        skos:Concept,
        dcat:Resource ;
    rdfs:label "Item I1351"@en-AU ;
    rdfs:comment "269 SMR  Delegation - GraphNodeID: I1351"@en-AU ;
    skos:definition "269 SMR  Delegation"@en-AU ;
    skos:narrower C1901A00006:1350 ;
    skos:prefLabel "Item I1351"@en-AU ;
    dcat:accessURL "https://www.legislation.gov.au/C1901A00006/2024-07-01/2024-07-01/text/original/epub/OEBPS/document_4/document_4.html#_Toc172628785"^^xsd:anyURI .

C1901A00006:1353 a legcons:Item,
        skos:Concept,
        dcat:Resource ;
    rdfs:label "Item I1353"@en-AU ;
    rdfs:comment "269 SMS  Form and manner of applications - GraphNodeID: I1353"@en-AU ;
    skos:definition "269 SMS  Form and manner of applications"@en-AU ;
    skos:narrower C1901A00006:1352 ;
    skos:prefLabel "Item I1353"@en-AU ;
    dcat:accessURL "https://www.legislation.gov.au/C1901A00006/2024-07-01/2024-07-01/text/original/epub/OEBPS/document_4/document_4.html#_Toc172628787"^^xsd:anyURI .

C1901A00006:1355 a legcons:Item,
        skos:Concept,
        dcat:Resource ;
    rdfs:label "Item I1355"@en-AU ;
    rdfs:comment "269 SMT  Disclosure of information - GraphNodeID: I1355"@en-AU ;
    skos:definition "269 SMT  Disclosure of information"@en-AU ;
    skos:narrower C1901A00006:1354 ;
    skos:prefLabel "Item I1355"@en-AU ;
    dcat:accessURL "https://www.legislation.gov.au/C1901A00006/2024-07-01/2024-07-01/text/original/epub/OEBPS/document_4/document_4.html#_Toc172628789"^^xsd:anyURI .

C1901A00006:1356 a legcons:Division,
        skos:Concept,
        dcat:Resource ;
    rdfs:label "Division D1356"@en-AU ;
    rdfs:comment "Division 1 Definitions and role of Minister - GraphNodeID: D1356"@en-AU ;
    skos:definition "Division 1 Definitions and role of Minister"@en-AU ;
    skos:narrower C1901A00006:1327 ;
    skos:prefLabel "Division D1356"@en-AU ;
    dcat:accessURL "https://www.legislation.gov.au/C1901A00006/2024-07-01/2024-07-01/text/original/epub/OEBPS/document_4/document_4.html#_Toc172628790"^^xsd:anyURI .

C1901A00006:1357 a legcons:Item,
        skos:Concept,
        dcat:Resource ;
    rdfs:label "Item I1357"@en-AU ;
    rdfs:comment "269 SN  What this Division is about - GraphNodeID: I1357"@en-AU ;
    skos:definition "269 SN  What this Division is about"@en-AU ;
    skos:narrower C1901A00006:1354 ;
    skos:prefLabel "Item I1357"@en-AU ;
    dcat:accessURL "https://www.legislation.gov.au/C1901A00006/2024-07-01/2024-07-01/text/original/epub/OEBPS/document_4/document_4.html#_Toc172628791"^^xsd:anyURI .

C1901A00006:1358 a legcons:Item,
        skos:Concept,
        dcat:Resource ;
    rdfs:label "Item I1358"@en-AU ;
    rdfs:comment "269 T  Definitions - GraphNodeID: I1358"@en-AU ;
    skos:definition "269 T  Definitions"@en-AU ;
    skos:narrower C1901A00006:1354 ;
    skos:prefLabel "Item I1358"@en-AU ;
    dcat:accessURL "https://www.legislation.gov.au/C1901A00006/2024-07-01/2024-07-01/text/original/epub/OEBPS/document_4/document_4.html#_Toc172628792"^^xsd:anyURI .

C1901A00006:1359 a legcons:Item,
        skos:Concept,
        dcat:Resource ;
    rdfs:label "Item I1359"@en-AU ;
    rdfs:comment "269 TAAA  Anti dumping measures not to apply to New Zealand originating goods - GraphNodeID: I1359"@en-AU ;
    skos:definition "269 TAAA  Anti dumping measures not to apply to New Zealand originating goods"@en-AU ;
    skos:narrower C1901A00006:1354 ;
    skos:prefLabel "Item I1359"@en-AU ;
    dcat:accessURL "https://www.legislation.gov.au/C1901A00006/2024-07-01/2024-07-01/text/original/epub/OEBPS/document_4/document_4.html#_Toc172628793"^^xsd:anyURI .

C1901A00006:136 a legcons:Item,
        skos:Concept,
        dcat:Resource ;
    rdfs:label "Item I136"@en-AU ;
    rdfs:comment "71 AAAH  Collectors response if a self assessed clearance declaration is communicated together with a cargo report - GraphNodeID: I136"@en-AU ;
    skos:definition "71 AAAH  Collectors response if a self assessed clearance declaration is communicated together with a cargo report"@en-AU ;
    skos:narrower C1901A00006:131 ;
    skos:prefLabel "Item I136"@en-AU ;
    dcat:accessURL "https://www.legislation.gov.au/C1901A00006/2024-07-01/2024-07-01/text/original/epub/OEBPS/document_1/document_1.html#_Toc172623110"^^xsd:anyURI .

C1901A00006:1360 a legcons:Item,
        skos:Concept,
        dcat:Resource ;
    rdfs:label "Item I1360"@en-AU ;
    rdfs:comment "269 TAAB  Member countries developing countries and special developing countries - GraphNodeID: I1360"@en-AU ;
    skos:definition "269 TAAB  Member countries developing countries and special developing countries"@en-AU ;
    skos:narrower C1901A00006:1354 ;
    skos:prefLabel "Item I1360"@en-AU ;
    dcat:accessURL "https://www.legislation.gov.au/C1901A00006/2024-07-01/2024-07-01/text/original/epub/OEBPS/document_4/document_4.html#_Toc172628794"^^xsd:anyURI .

C1901A00006:1361 a legcons:Item,
        skos:Concept,
        dcat:Resource ;
    rdfs:label "Item I1361"@en-AU ;
    rdfs:comment "269 TAAC  Definitioncountervailable subsidy - GraphNodeID: I1361"@en-AU ;
    skos:definition "269 TAAC  Definitioncountervailable subsidy"@en-AU ;
    skos:narrower C1901A00006:1354 ;
    skos:prefLabel "Item I1361"@en-AU ;
    dcat:accessURL "https://www.legislation.gov.au/C1901A00006/2024-07-01/2024-07-01/text/original/epub/OEBPS/document_4/document_4.html#_Toc172628795"^^xsd:anyURI .

C1901A00006:1362 a legcons:Item,
        skos:Concept,
        dcat:Resource ;
    rdfs:label "Item I1362"@en-AU ;
    rdfs:comment "269 TAACA  Determination of countervailable subsidy if non cooperation by relevant entities - GraphNodeID: I1362"@en-AU ;
    skos:definition "269 TAACA  Determination of countervailable subsidy if non cooperation by relevant entities"@en-AU ;
    skos:narrower C1901A00006:1354 ;
    skos:prefLabel "Item I1362"@en-AU ;
    dcat:accessURL "https://www.legislation.gov.au/C1901A00006/2024-07-01/2024-07-01/text/original/epub/OEBPS/document_4/document_4.html#_Toc172628796"^^xsd:anyURI .

C1901A00006:1363 a legcons:Item,
        skos:Concept,
        dcat:Resource ;
    rdfs:label "Item I1363"@en-AU ;
    rdfs:comment "269 TAAD  Ordinary course of trade - GraphNodeID: I1363"@en-AU ;
    skos:definition "269 TAAD  Ordinary course of trade"@en-AU ;
    skos:narrower C1901A00006:1354 ;
    skos:prefLabel "Item I1363"@en-AU ;
    dcat:accessURL "https://www.legislation.gov.au/C1901A00006/2024-07-01/2024-07-01/text/original/epub/OEBPS/document_4/document_4.html#_Toc172628797"^^xsd:anyURI .

C1901A00006:1364 a legcons:Item,
        skos:Concept,
        dcat:Resource ;
    rdfs:label "Item I1364"@en-AU ;
    rdfs:comment "269 TAA  Arms length transactions - GraphNodeID: I1364"@en-AU ;
    skos:definition "269 TAA  Arms length transactions"@en-AU ;
    skos:narrower C1901A00006:1354 ;
    skos:prefLabel "Item I1364"@en-AU ;
    dcat:accessURL "https://www.legislation.gov.au/C1901A00006/2024-07-01/2024-07-01/text/original/epub/OEBPS/document_4/document_4.html#_Toc172628798"^^xsd:anyURI .

C1901A00006:1365 a legcons:Item,
        skos:Concept,
        dcat:Resource ;
    rdfs:label "Item I1365"@en-AU ;
    rdfs:comment "269 TAB  Export price - GraphNodeID: I1365"@en-AU ;
    skos:definition "269 TAB  Export price"@en-AU ;
    skos:narrower C1901A00006:1354 ;
    skos:prefLabel "Item I1365"@en-AU ;
    dcat:accessURL "https://www.legislation.gov.au/C1901A00006/2024-07-01/2024-07-01/text/original/epub/OEBPS/document_4/document_4.html#_Toc172628799"^^xsd:anyURI .

C1901A00006:1366 a legcons:Item,
        skos:Concept,
        dcat:Resource ;
    rdfs:label "Item I1366"@en-AU ;
    rdfs:comment "269 TAC  Normal value of goods - GraphNodeID: I1366"@en-AU ;
    skos:definition "269 TAC  Normal value of goods"@en-AU ;
    skos:narrower C1901A00006:1354 ;
    skos:prefLabel "Item I1366"@en-AU ;
    dcat:accessURL "https://www.legislation.gov.au/C1901A00006/2024-07-01/2024-07-01/text/original/epub/OEBPS/document_4/document_4.html#_Toc172628800"^^xsd:anyURI .

C1901A00006:1367 a legcons:Item,
        skos:Concept,
        dcat:Resource ;
    rdfs:label "Item I1367"@en-AU ;
    rdfs:comment "269 TACAA  Sampling - GraphNodeID: I1367"@en-AU ;
    skos:definition "269 TACAA  Sampling"@en-AU ;
    skos:narrower C1901A00006:1354 ;
    skos:prefLabel "Item I1367"@en-AU ;
    dcat:accessURL "https://www.legislation.gov.au/C1901A00006/2024-07-01/2024-07-01/text/original/epub/OEBPS/document_4/document_4.html#_Toc172628801"^^xsd:anyURI .

C1901A00006:1368 a legcons:Item,
        skos:Concept,
        dcat:Resource ;
    rdfs:label "Item I1368"@en-AU ;
    rdfs:comment "269 TACAB  Dumping duty noticeexport prices and normal values for different categories of exporters - GraphNodeID: I1368"@en-AU ;
    skos:definition "269 TACAB  Dumping duty noticeexport prices and normal values for different categories of exporters"@en-AU ;
    skos:narrower C1901A00006:1354 ;
    skos:prefLabel "Item I1368"@en-AU ;
    dcat:accessURL "https://www.legislation.gov.au/C1901A00006/2024-07-01/2024-07-01/text/original/epub/OEBPS/document_4/document_4.html#_Toc172628802"^^xsd:anyURI .

C1901A00006:1369 a legcons:Item,
        skos:Concept,
        dcat:Resource ;
    rdfs:label "Item I1369"@en-AU ;
    rdfs:comment "269 TACA  Non injurious price - GraphNodeID: I1369"@en-AU ;
    skos:definition "269 TACA  Non injurious price"@en-AU ;
    skos:narrower C1901A00006:1354 ;
    skos:prefLabel "Item I1369"@en-AU ;
    dcat:accessURL "https://www.legislation.gov.au/C1901A00006/2024-07-01/2024-07-01/text/original/epub/OEBPS/document_4/document_4.html#_Toc172628803"^^xsd:anyURI .

C1901A00006:137 a legcons:Item,
        skos:Concept,
        dcat:Resource ;
    rdfs:label "Item I137"@en-AU ;
    rdfs:comment "71 AAAI  Authority to deal with goods covered by a self assessed clearance declaration - GraphNodeID: I137"@en-AU ;
    skos:definition "71 AAAI  Authority to deal with goods covered by a self assessed clearance declaration"@en-AU ;
    skos:narrower C1901A00006:131 ;
    skos:prefLabel "Item I137"@en-AU ;
    dcat:accessURL "https://www.legislation.gov.au/C1901A00006/2024-07-01/2024-07-01/text/original/epub/OEBPS/document_1/document_1.html#_Toc172623111"^^xsd:anyURI .

C1901A00006:1370 a legcons:Item,
        skos:Concept,
        dcat:Resource ;
    rdfs:label "Item I1370"@en-AU ;
    rdfs:comment "269 TACB  Working out whether dumping has occurred and levels of dumping - GraphNodeID: I1370"@en-AU ;
    skos:definition "269 TACB  Working out whether dumping has occurred and levels of dumping"@en-AU ;
    skos:narrower C1901A00006:1354 ;
    skos:prefLabel "Item I1370"@en-AU ;
    dcat:accessURL "https://www.legislation.gov.au/C1901A00006/2024-07-01/2024-07-01/text/original/epub/OEBPS/document_4/document_4.html#_Toc172628804"^^xsd:anyURI .

C1901A00006:1371 a legcons:Item,
        skos:Concept,
        dcat:Resource ;
    rdfs:label "Item I1371"@en-AU ;
    rdfs:comment "269 TACC  Working out whether a financial contribution or income or price support confers a benefit - GraphNodeID: I1371"@en-AU ;
    skos:definition "269 TACC  Working out whether a financial contribution or income or price support confers a benefit"@en-AU ;
    skos:narrower C1901A00006:1354 ;
    skos:prefLabel "Item I1371"@en-AU ;
    dcat:accessURL "https://www.legislation.gov.au/C1901A00006/2024-07-01/2024-07-01/text/original/epub/OEBPS/document_4/document_4.html#_Toc172628805"^^xsd:anyURI .

C1901A00006:1372 a legcons:Item,
        skos:Concept,
        dcat:Resource ;
    rdfs:label "Item I1372"@en-AU ;
    rdfs:comment "269 TACD  Amount of countervailable subsidy - GraphNodeID: I1372"@en-AU ;
    skos:definition "269 TACD  Amount of countervailable subsidy"@en-AU ;
    skos:narrower C1901A00006:1354 ;
    skos:prefLabel "Item I1372"@en-AU ;
    dcat:accessURL "https://www.legislation.gov.au/C1901A00006/2024-07-01/2024-07-01/text/original/epub/OEBPS/document_4/document_4.html#_Toc172628806"^^xsd:anyURI .

C1901A00006:1373 a legcons:Item,
        skos:Concept,
        dcat:Resource ;
    rdfs:label "Item I1373"@en-AU ;
    rdfs:comment "269 TAE  Material injury to industry - GraphNodeID: I1373"@en-AU ;
    skos:definition "269 TAE  Material injury to industry"@en-AU ;
    skos:narrower C1901A00006:1354 ;
    skos:prefLabel "Item I1373"@en-AU ;
    dcat:accessURL "https://www.legislation.gov.au/C1901A00006/2024-07-01/2024-07-01/text/original/epub/OEBPS/document_4/document_4.html#_Toc172628807"^^xsd:anyURI .

C1901A00006:1374 a legcons:Item,
        skos:Concept,
        dcat:Resource ;
    rdfs:label "Item I1374"@en-AU ;
    rdfs:comment "269 TAF  Currency conversion - GraphNodeID: I1374"@en-AU ;
    skos:definition "269 TAF  Currency conversion"@en-AU ;
    skos:narrower C1901A00006:1354 ;
    skos:prefLabel "Item I1374"@en-AU ;
    dcat:accessURL "https://www.legislation.gov.au/C1901A00006/2024-07-01/2024-07-01/text/original/epub/OEBPS/document_4/document_4.html#_Toc172628808"^^xsd:anyURI .

C1901A00006:1375 a legcons:Item,
        skos:Concept,
        dcat:Resource ;
    rdfs:label "Item I1375"@en-AU ;
    rdfs:comment "269 TAG  Minister may take anti dumping measures on own initiative - GraphNodeID: I1375"@en-AU ;
    skos:definition "269 TAG  Minister may take anti dumping measures on own initiative"@en-AU ;
    skos:narrower C1901A00006:1354 ;
    skos:prefLabel "Item I1375"@en-AU ;
    dcat:accessURL "https://www.legislation.gov.au/C1901A00006/2024-07-01/2024-07-01/text/original/epub/OEBPS/document_4/document_4.html#_Toc172628809"^^xsd:anyURI .

C1901A00006:1376 a legcons:Item,
        skos:Concept,
        dcat:Resource ;
    rdfs:label "Item I1376"@en-AU ;
    rdfs:comment "269 TAH  Minister may delegate functions and powers to Commissioner or Commission staff members - GraphNodeID: I1376"@en-AU ;
    skos:definition "269 TAH  Minister may delegate functions and powers to Commissioner or Commission staff members"@en-AU ;
    skos:narrower C1901A00006:1354 ;
    skos:prefLabel "Item I1376"@en-AU ;
    dcat:accessURL "https://www.legislation.gov.au/C1901A00006/2024-07-01/2024-07-01/text/original/epub/OEBPS/document_4/document_4.html#_Toc172628810"^^xsd:anyURI .

C1901A00006:1377 a legcons:Item,
        skos:Concept,
        dcat:Resource ;
    rdfs:label "Item I1377"@en-AU ;
    rdfs:comment "269 TA  Minister may give directions to Commissioner in relation to powers and duties under this Part - GraphNodeID: I1377"@en-AU ;
    skos:definition "269 TA  Minister may give directions to Commissioner in relation to powers and duties under this Part"@en-AU ;
    skos:narrower C1901A00006:1354 ;
    skos:prefLabel "Item I1377"@en-AU ;
    dcat:accessURL "https://www.legislation.gov.au/C1901A00006/2024-07-01/2024-07-01/text/original/epub/OEBPS/document_4/document_4.html#_Toc172628811"^^xsd:anyURI .

C1901A00006:1378 a legcons:Division,
        skos:Concept,
        dcat:Resource ;
    rdfs:label "Division D1378"@en-AU ;
    rdfs:comment "Division 2 Consideration of anti dumping matters by the Commissioner - GraphNodeID: D1378"@en-AU ;
    skos:definition "Division 2 Consideration of anti dumping matters by the Commissioner"@en-AU ;
    skos:narrower C1901A00006:1327 ;
    skos:prefLabel "Division D1378"@en-AU ;
    dcat:accessURL "https://www.legislation.gov.au/C1901A00006/2024-07-01/2024-07-01/text/original/epub/OEBPS/document_4/document_4.html#_Toc172628812"^^xsd:anyURI .

C1901A00006:1379 a legcons:Item,
        skos:Concept,
        dcat:Resource ;
    rdfs:label "Item I1379"@en-AU ;
    rdfs:comment "269 TBA  What this Division is about - GraphNodeID: I1379"@en-AU ;
    skos:definition "269 TBA  What this Division is about"@en-AU ;
    skos:narrower C1901A00006:1354 ;
    skos:prefLabel "Item I1379"@en-AU ;
    dcat:accessURL "https://www.legislation.gov.au/C1901A00006/2024-07-01/2024-07-01/text/original/epub/OEBPS/document_4/document_4.html#_Toc172628813"^^xsd:anyURI .

C1901A00006:138 a legcons:Item,
        skos:Concept,
        dcat:Resource ;
    rdfs:label "Item I138"@en-AU ;
    rdfs:comment "71 AAAJ  Contents of authority to deal with specified low value goods - GraphNodeID: I138"@en-AU ;
    skos:definition "71 AAAJ  Contents of authority to deal with specified low value goods"@en-AU ;
    skos:narrower C1901A00006:131 ;
    skos:prefLabel "Item I138"@en-AU ;
    dcat:accessURL "https://www.legislation.gov.au/C1901A00006/2024-07-01/2024-07-01/text/original/epub/OEBPS/document_1/document_1.html#_Toc172623112"^^xsd:anyURI .

C1901A00006:1380 a legcons:Item,
        skos:Concept,
        dcat:Resource ;
    rdfs:label "Item I1380"@en-AU ;
    rdfs:comment "269 TB  Application for action under Dumping Duty Act - GraphNodeID: I1380"@en-AU ;
    skos:definition "269 TB  Application for action under Dumping Duty Act"@en-AU ;
    skos:narrower C1901A00006:1354 ;
    skos:prefLabel "Item I1380"@en-AU ;
    dcat:accessURL "https://www.legislation.gov.au/C1901A00006/2024-07-01/2024-07-01/text/original/epub/OEBPS/document_4/document_4.html#_Toc172628814"^^xsd:anyURI .

C1901A00006:1381 a legcons:Item,
        skos:Concept,
        dcat:Resource ;
    rdfs:label "Item I1381"@en-AU ;
    rdfs:comment "269 TC  Consideration of application - GraphNodeID: I1381"@en-AU ;
    skos:definition "269 TC  Consideration of application"@en-AU ;
    skos:narrower C1901A00006:1354 ;
    skos:prefLabel "Item I1381"@en-AU ;
    dcat:accessURL "https://www.legislation.gov.au/C1901A00006/2024-07-01/2024-07-01/text/original/epub/OEBPS/document_4/document_4.html#_Toc172628815"^^xsd:anyURI .

C1901A00006:1382 a legcons:Item,
        skos:Concept,
        dcat:Resource ;
    rdfs:label "Item I1382"@en-AU ;
    rdfs:comment "269 TD  Preliminary affirmative determinations - GraphNodeID: I1382"@en-AU ;
    skos:definition "269 TD  Preliminary affirmative determinations"@en-AU ;
    skos:narrower C1901A00006:1354 ;
    skos:prefLabel "Item I1382"@en-AU ;
    dcat:accessURL "https://www.legislation.gov.au/C1901A00006/2024-07-01/2024-07-01/text/original/epub/OEBPS/document_4/document_4.html#_Toc172628816"^^xsd:anyURI .

C1901A00006:1383 a legcons:Item,
        skos:Concept,
        dcat:Resource ;
    rdfs:label "Item I1383"@en-AU ;
    rdfs:comment "269 TDAA  Statement of essential facts in relation to investigation of application under section 269 TB - GraphNodeID: I1383"@en-AU ;
    skos:definition "269 TDAA  Statement of essential facts in relation to investigation of application under section 269 TB"@en-AU ;
    skos:narrower C1901A00006:1354 ;
    skos:prefLabel "Item I1383"@en-AU ;
    dcat:accessURL "https://www.legislation.gov.au/C1901A00006/2024-07-01/2024-07-01/text/original/epub/OEBPS/document_4/document_4.html#_Toc172628817"^^xsd:anyURI .

C1901A00006:1384 a legcons:Item,
        skos:Concept,
        dcat:Resource ;
    rdfs:label "Item I1384"@en-AU ;
    rdfs:comment "269 TDA  Termination of investigations - GraphNodeID: I1384"@en-AU ;
    skos:definition "269 TDA  Termination of investigations"@en-AU ;
    skos:narrower C1901A00006:1354 ;
    skos:prefLabel "Item I1384"@en-AU ;
    dcat:accessURL "https://www.legislation.gov.au/C1901A00006/2024-07-01/2024-07-01/text/original/epub/OEBPS/document_4/document_4.html#_Toc172628818"^^xsd:anyURI .

C1901A00006:1385 a legcons:Item,
        skos:Concept,
        dcat:Resource ;
    rdfs:label "Item I1385"@en-AU ;
    rdfs:comment "269 TE  Commissioner to have regard to same considerations as Minister - GraphNodeID: I1385"@en-AU ;
    skos:definition "269 TE  Commissioner to have regard to same considerations as Minister"@en-AU ;
    skos:narrower C1901A00006:1354 ;
    skos:prefLabel "Item I1385"@en-AU ;
    dcat:accessURL "https://www.legislation.gov.au/C1901A00006/2024-07-01/2024-07-01/text/original/epub/OEBPS/document_4/document_4.html#_Toc172628819"^^xsd:anyURI .

C1901A00006:1386 a legcons:Item,
        skos:Concept,
        dcat:Resource ;
    rdfs:label "Item I1386"@en-AU ;
    rdfs:comment "269 TEA  Report to Minister concerning publication of notices under this Part - GraphNodeID: I1386"@en-AU ;
    skos:definition "269 TEA  Report to Minister concerning publication of notices under this Part"@en-AU ;
    skos:narrower C1901A00006:1354 ;
    skos:prefLabel "Item I1386"@en-AU ;
    dcat:accessURL "https://www.legislation.gov.au/C1901A00006/2024-07-01/2024-07-01/text/original/epub/OEBPS/document_4/document_4.html#_Toc172628820"^^xsd:anyURI .

C1901A00006:1387 a legcons:Item,
        skos:Concept,
        dcat:Resource ;
    rdfs:label "Item I1387"@en-AU ;
    rdfs:comment "269 TEB  Commissioner recommendations concerning undertakings offered after preliminary affirmative determination - GraphNodeID: I1387"@en-AU ;
    skos:definition "269 TEB  Commissioner recommendations concerning undertakings offered after preliminary affirmative determination"@en-AU ;
    skos:narrower C1901A00006:1354 ;
    skos:prefLabel "Item I1387"@en-AU ;
    dcat:accessURL "https://www.legislation.gov.au/C1901A00006/2024-07-01/2024-07-01/text/original/epub/OEBPS/document_4/document_4.html#_Toc172628821"^^xsd:anyURI .

C1901A00006:1388 a legcons:Division,
        skos:Concept,
        dcat:Resource ;
    rdfs:label "Division D1388"@en-AU ;
    rdfs:comment "Division 3 Consideration of anti dumping matters by the Minister - GraphNodeID: D1388"@en-AU ;
    skos:definition "Division 3 Consideration of anti dumping matters by the Minister"@en-AU ;
    skos:narrower C1901A00006:1327 ;
    skos:prefLabel "Division D1388"@en-AU ;
    dcat:accessURL "https://www.legislation.gov.au/C1901A00006/2024-07-01/2024-07-01/text/original/epub/OEBPS/document_4/document_4.html#_Toc172628822"^^xsd:anyURI .

C1901A00006:1389 a legcons:Item,
        skos:Concept,
        dcat:Resource ;
    rdfs:label "Item I1389"@en-AU ;
    rdfs:comment "269 TF  What this Division is about - GraphNodeID: I1389"@en-AU ;
    skos:definition "269 TF  What this Division is about"@en-AU ;
    skos:narrower C1901A00006:1354 ;
    skos:prefLabel "Item I1389"@en-AU ;
    dcat:accessURL "https://www.legislation.gov.au/C1901A00006/2024-07-01/2024-07-01/text/original/epub/OEBPS/document_4/document_4.html#_Toc172628823"^^xsd:anyURI .

C1901A00006:139 a legcons:Item,
        skos:Concept,
        dcat:Resource ;
    rdfs:label "Item I139"@en-AU ;
    rdfs:comment "71 AAAK  No authority to deal with specified low value goods while subject to a direction to hold or further examine - GraphNodeID: I139"@en-AU ;
    skos:definition "71 AAAK  No authority to deal with specified low value goods while subject to a direction to hold or further examine"@en-AU ;
    skos:narrower C1901A00006:131 ;
    skos:prefLabel "Item I139"@en-AU ;
    dcat:accessURL "https://www.legislation.gov.au/C1901A00006/2024-07-01/2024-07-01/text/original/epub/OEBPS/document_1/document_1.html#_Toc172623113"^^xsd:anyURI .

C1901A00006:1390 a legcons:Item,
        skos:Concept,
        dcat:Resource ;
    rdfs:label "Item I1390"@en-AU ;
    rdfs:comment "269 TG  Dumping duties - GraphNodeID: I1390"@en-AU ;
    skos:definition "269 TG  Dumping duties"@en-AU ;
    skos:narrower C1901A00006:1354 ;
    skos:prefLabel "Item I1390"@en-AU ;
    dcat:accessURL "https://www.legislation.gov.au/C1901A00006/2024-07-01/2024-07-01/text/original/epub/OEBPS/document_4/document_4.html#_Toc172628824"^^xsd:anyURI .

C1901A00006:1391 a legcons:Item,
        skos:Concept,
        dcat:Resource ;
    rdfs:label "Item I1391"@en-AU ;
    rdfs:comment "269 TH  Third country dumping duties - GraphNodeID: I1391"@en-AU ;
    skos:definition "269 TH  Third country dumping duties"@en-AU ;
    skos:narrower C1901A00006:1354 ;
    skos:prefLabel "Item I1391"@en-AU ;
    dcat:accessURL "https://www.legislation.gov.au/C1901A00006/2024-07-01/2024-07-01/text/original/epub/OEBPS/document_4/document_4.html#_Toc172628825"^^xsd:anyURI .

C1901A00006:1392 a legcons:Item,
        skos:Concept,
        dcat:Resource ;
    rdfs:label "Item I1392"@en-AU ;
    rdfs:comment "269 TJ  Countervailing duties - GraphNodeID: I1392"@en-AU ;
    skos:definition "269 TJ  Countervailing duties"@en-AU ;
    skos:narrower C1901A00006:1354 ;
    skos:prefLabel "Item I1392"@en-AU ;
    dcat:accessURL "https://www.legislation.gov.au/C1901A00006/2024-07-01/2024-07-01/text/original/epub/OEBPS/document_4/document_4.html#_Toc172628826"^^xsd:anyURI .

C1901A00006:1393 a legcons:Item,
        skos:Concept,
        dcat:Resource ;
    rdfs:label "Item I1393"@en-AU ;
    rdfs:comment "269 TJA  Concurrent dumping and subsidy - GraphNodeID: I1393"@en-AU ;
    skos:definition "269 TJA  Concurrent dumping and subsidy"@en-AU ;
    skos:narrower C1901A00006:1354 ;
    skos:prefLabel "Item I1393"@en-AU ;
    dcat:accessURL "https://www.legislation.gov.au/C1901A00006/2024-07-01/2024-07-01/text/original/epub/OEBPS/document_4/document_4.html#_Toc172628827"^^xsd:anyURI .

C1901A00006:1394 a legcons:Item,
        skos:Concept,
        dcat:Resource ;
    rdfs:label "Item I1394"@en-AU ;
    rdfs:comment "269 TK  Third country countervailing duties - GraphNodeID: I1394"@en-AU ;
    skos:definition "269 TK  Third country countervailing duties"@en-AU ;
    skos:narrower C1901A00006:1354 ;
    skos:prefLabel "Item I1394"@en-AU ;
    dcat:accessURL "https://www.legislation.gov.au/C1901A00006/2024-07-01/2024-07-01/text/original/epub/OEBPS/document_4/document_4.html#_Toc172628828"^^xsd:anyURI .

C1901A00006:1395 a legcons:Item,
        skos:Concept,
        dcat:Resource ;
    rdfs:label "Item I1395"@en-AU ;
    rdfs:comment "269 TL  Minister to give public notice not to impose duty - GraphNodeID: I1395"@en-AU ;
    skos:definition "269 TL  Minister to give public notice not to impose duty"@en-AU ;
    skos:narrower C1901A00006:1354 ;
    skos:prefLabel "Item I1395"@en-AU ;
    dcat:accessURL "https://www.legislation.gov.au/C1901A00006/2024-07-01/2024-07-01/text/original/epub/OEBPS/document_4/document_4.html#_Toc172628829"^^xsd:anyURI .

C1901A00006:1396 a legcons:Item,
        skos:Concept,
        dcat:Resource ;
    rdfs:label "Item I1396"@en-AU ;
    rdfs:comment "269 TLA  Time limit for Minister to make certain decisions - GraphNodeID: I1396"@en-AU ;
    skos:definition "269 TLA  Time limit for Minister to make certain decisions"@en-AU ;
    skos:narrower C1901A00006:1354 ;
    skos:prefLabel "Item I1396"@en-AU ;
    dcat:accessURL "https://www.legislation.gov.au/C1901A00006/2024-07-01/2024-07-01/text/original/epub/OEBPS/document_4/document_4.html#_Toc172628830"^^xsd:anyURI .

C1901A00006:1397 a legcons:Item,
        skos:Concept,
        dcat:Resource ;
    rdfs:label "Item I1397"@en-AU ;
    rdfs:comment "269 TM  Periods during which certain notices and undertakings to remain in force - GraphNodeID: I1397"@en-AU ;
    skos:definition "269 TM  Periods during which certain notices and undertakings to remain in force"@en-AU ;
    skos:narrower C1901A00006:1354 ;
    skos:prefLabel "Item I1397"@en-AU ;
    dcat:accessURL "https://www.legislation.gov.au/C1901A00006/2024-07-01/2024-07-01/text/original/epub/OEBPS/document_4/document_4.html#_Toc172628831"^^xsd:anyURI .

C1901A00006:1398 a legcons:Item,
        skos:Concept,
        dcat:Resource ;
    rdfs:label "Item I1398"@en-AU ;
    rdfs:comment "269 TN  Retrospective notices - GraphNodeID: I1398"@en-AU ;
    skos:definition "269 TN  Retrospective notices"@en-AU ;
    skos:narrower C1901A00006:1354 ;
    skos:prefLabel "Item I1398"@en-AU ;
    dcat:accessURL "https://www.legislation.gov.au/C1901A00006/2024-07-01/2024-07-01/text/original/epub/OEBPS/document_4/document_4.html#_Toc172628832"^^xsd:anyURI .

C1901A00006:1399 a legcons:Item,
        skos:Concept,
        dcat:Resource ;
    rdfs:label "Item I1399"@en-AU ;
    rdfs:comment "269 TP  Power to specify goods - GraphNodeID: I1399"@en-AU ;
    skos:definition "269 TP  Power to specify goods"@en-AU ;
    skos:narrower C1901A00006:1354 ;
    skos:prefLabel "Item I1399"@en-AU ;
    dcat:accessURL "https://www.legislation.gov.au/C1901A00006/2024-07-01/2024-07-01/text/original/epub/OEBPS/document_4/document_4.html#_Toc172628833"^^xsd:anyURI .

C1901A00006:140 a legcons:Item,
        skos:Concept,
        dcat:Resource ;
    rdfs:label "Item I140"@en-AU ;
    rdfs:comment "71 AAAL  No authority to deal with specified low value goods unless duty etc paid - GraphNodeID: I140"@en-AU ;
    skos:definition "71 AAAL  No authority to deal with specified low value goods unless duty etc paid"@en-AU ;
    skos:narrower C1901A00006:131 ;
    skos:prefLabel "Item I140"@en-AU ;
    dcat:accessURL "https://www.legislation.gov.au/C1901A00006/2024-07-01/2024-07-01/text/original/epub/OEBPS/document_1/document_1.html#_Toc172623114"^^xsd:anyURI .

C1901A00006:1400 a legcons:Item,
        skos:Concept,
        dcat:Resource ;
    rdfs:label "Item I1400"@en-AU ;
    rdfs:comment "269 U  Inquiries in relation to undertakings - GraphNodeID: I1400"@en-AU ;
    skos:definition "269 U  Inquiries in relation to undertakings"@en-AU ;
    skos:narrower C1901A00006:1354 ;
    skos:prefLabel "Item I1400"@en-AU ;
    dcat:accessURL "https://www.legislation.gov.au/C1901A00006/2024-07-01/2024-07-01/text/original/epub/OEBPS/document_4/document_4.html#_Toc172628834"^^xsd:anyURI .

C1901A00006:1401 a legcons:Division,
        skos:Concept,
        dcat:Resource ;
    rdfs:label "Division D1401"@en-AU ;
    rdfs:comment "Division 4 Dumping duty or countervailing duty assessment - GraphNodeID: D1401"@en-AU ;
    skos:definition "Division 4 Dumping duty or countervailing duty assessment"@en-AU ;
    skos:narrower C1901A00006:1327 ;
    skos:prefLabel "Division D1401"@en-AU ;
    dcat:accessURL "https://www.legislation.gov.au/C1901A00006/2024-07-01/2024-07-01/text/original/epub/OEBPS/document_4/document_4.html#_Toc172628835"^^xsd:anyURI .

C1901A00006:1402 a legcons:Item,
        skos:Concept,
        dcat:Resource ;
    rdfs:label "Item I1402"@en-AU ;
    rdfs:comment "269 UA  What this Division is about - GraphNodeID: I1402"@en-AU ;
    skos:definition "269 UA  What this Division is about"@en-AU ;
    skos:narrower C1901A00006:1354 ;
    skos:prefLabel "Item I1402"@en-AU ;
    dcat:accessURL "https://www.legislation.gov.au/C1901A00006/2024-07-01/2024-07-01/text/original/epub/OEBPS/document_4/document_4.html#_Toc172628836"^^xsd:anyURI .

C1901A00006:1403 a legcons:Item,
        skos:Concept,
        dcat:Resource ;
    rdfs:label "Item I1403"@en-AU ;
    rdfs:comment "269 V  Importers may apply for duty assessment in certain circumstances - GraphNodeID: I1403"@en-AU ;
    skos:definition "269 V  Importers may apply for duty assessment in certain circumstances"@en-AU ;
    skos:narrower C1901A00006:1354 ;
    skos:prefLabel "Item I1403"@en-AU ;
    dcat:accessURL "https://www.legislation.gov.au/C1901A00006/2024-07-01/2024-07-01/text/original/epub/OEBPS/document_4/document_4.html#_Toc172628837"^^xsd:anyURI .

C1901A00006:1404 a legcons:Item,
        skos:Concept,
        dcat:Resource ;
    rdfs:label "Item I1404"@en-AU ;
    rdfs:comment "269 W  Manner of making applications for duty assessment - GraphNodeID: I1404"@en-AU ;
    skos:definition "269 W  Manner of making applications for duty assessment"@en-AU ;
    skos:narrower C1901A00006:1354 ;
    skos:prefLabel "Item I1404"@en-AU ;
    dcat:accessURL "https://www.legislation.gov.au/C1901A00006/2024-07-01/2024-07-01/text/original/epub/OEBPS/document_4/document_4.html#_Toc172628838"^^xsd:anyURI .

C1901A00006:1405 a legcons:Item,
        skos:Concept,
        dcat:Resource ;
    rdfs:label "Item I1405"@en-AU ;
    rdfs:comment "269 X  Consideration of duty assessment applications - GraphNodeID: I1405"@en-AU ;
    skos:definition "269 X  Consideration of duty assessment applications"@en-AU ;
    skos:narrower C1901A00006:1354 ;
    skos:prefLabel "Item I1405"@en-AU ;
    dcat:accessURL "https://www.legislation.gov.au/C1901A00006/2024-07-01/2024-07-01/text/original/epub/OEBPS/document_4/document_4.html#_Toc172628839"^^xsd:anyURI .

C1901A00006:1406 a legcons:Item,
        skos:Concept,
        dcat:Resource ;
    rdfs:label "Item I1406"@en-AU ;
    rdfs:comment "269 Y  Duty assessments - GraphNodeID: I1406"@en-AU ;
    skos:definition "269 Y  Duty assessments"@en-AU ;
    skos:narrower C1901A00006:1354 ;
    skos:prefLabel "Item I1406"@en-AU ;
    dcat:accessURL "https://www.legislation.gov.au/C1901A00006/2024-07-01/2024-07-01/text/original/epub/OEBPS/document_4/document_4.html#_Toc172628840"^^xsd:anyURI .

C1901A00006:1407 a legcons:Item,
        skos:Concept,
        dcat:Resource ;
    rdfs:label "Item I1407"@en-AU ;
    rdfs:comment "269 YA  Rejection etc of application for duty assessment - GraphNodeID: I1407"@en-AU ;
    skos:definition "269 YA  Rejection etc of application for duty assessment"@en-AU ;
    skos:narrower C1901A00006:1354 ;
    skos:prefLabel "Item I1407"@en-AU ;
    dcat:accessURL "https://www.legislation.gov.au/C1901A00006/2024-07-01/2024-07-01/text/original/epub/OEBPS/document_4/document_4.html#_Toc172628841"^^xsd:anyURI .

C1901A00006:1408 a legcons:Division,
        skos:Concept,
        dcat:Resource ;
    rdfs:label "Division D1408"@en-AU ;
    rdfs:comment "Division 5 Review of anti dumping measures - GraphNodeID: D1408"@en-AU ;
    skos:definition "Division 5 Review of anti dumping measures"@en-AU ;
    skos:narrower C1901A00006:1327 ;
    skos:prefLabel "Division D1408"@en-AU ;
    dcat:accessURL "https://www.legislation.gov.au/C1901A00006/2024-07-01/2024-07-01/text/original/epub/OEBPS/document_4/document_4.html#_Toc172628842"^^xsd:anyURI .

C1901A00006:1409 a legcons:Item,
        skos:Concept,
        dcat:Resource ;
    rdfs:label "Item I1409"@en-AU ;
    rdfs:comment "269 Z  What this Division is about - GraphNodeID: I1409"@en-AU ;
    skos:definition "269 Z  What this Division is about"@en-AU ;
    skos:narrower C1901A00006:1354 ;
    skos:prefLabel "Item I1409"@en-AU ;
    dcat:accessURL "https://www.legislation.gov.au/C1901A00006/2024-07-01/2024-07-01/text/original/epub/OEBPS/document_4/document_4.html#_Toc172628843"^^xsd:anyURI .

C1901A00006:141 a legcons:Item,
        skos:Concept,
        dcat:Resource ;
    rdfs:label "Item I141"@en-AU ;
    rdfs:comment "71 AAAM  Suspension of authority to deal with specified low value goods - GraphNodeID: I141"@en-AU ;
    skos:definition "71 AAAM  Suspension of authority to deal with specified low value goods"@en-AU ;
    skos:narrower C1901A00006:131 ;
    skos:prefLabel "Item I141"@en-AU ;
    dcat:accessURL "https://www.legislation.gov.au/C1901A00006/2024-07-01/2024-07-01/text/original/epub/OEBPS/document_1/document_1.html#_Toc172623115"^^xsd:anyURI .

C1901A00006:1410 a legcons:Item,
        skos:Concept,
        dcat:Resource ;
    rdfs:label "Item I1410"@en-AU ;
    rdfs:comment "269 ZA  Applications and requests for review of anti dumping measures - GraphNodeID: I1410"@en-AU ;
    skos:definition "269 ZA  Applications and requests for review of anti dumping measures"@en-AU ;
    skos:narrower C1901A00006:1354 ;
    skos:prefLabel "Item I1410"@en-AU ;
    dcat:accessURL "https://www.legislation.gov.au/C1901A00006/2024-07-01/2024-07-01/text/original/epub/OEBPS/document_4/document_4.html#_Toc172628844"^^xsd:anyURI .

C1901A00006:1411 a legcons:Item,
        skos:Concept,
        dcat:Resource ;
    rdfs:label "Item I1411"@en-AU ;
    rdfs:comment "269 ZB  Content and lodgment of applications for review of anti dumping measures - GraphNodeID: I1411"@en-AU ;
    skos:definition "269 ZB  Content and lodgment of applications for review of anti dumping measures"@en-AU ;
    skos:narrower C1901A00006:1354 ;
    skos:prefLabel "Item I1411"@en-AU ;
    dcat:accessURL "https://www.legislation.gov.au/C1901A00006/2024-07-01/2024-07-01/text/original/epub/OEBPS/document_4/document_4.html#_Toc172628845"^^xsd:anyURI .

C1901A00006:1412 a legcons:Item,
        skos:Concept,
        dcat:Resource ;
    rdfs:label "Item I1412"@en-AU ;
    rdfs:comment "269 ZC  Consideration of applications and requests for review - GraphNodeID: I1412"@en-AU ;
    skos:definition "269 ZC  Consideration of applications and requests for review"@en-AU ;
    skos:narrower C1901A00006:1354 ;
    skos:prefLabel "Item I1412"@en-AU ;
    dcat:accessURL "https://www.legislation.gov.au/C1901A00006/2024-07-01/2024-07-01/text/original/epub/OEBPS/document_4/document_4.html#_Toc172628846"^^xsd:anyURI .

C1901A00006:1413 a legcons:Item,
        skos:Concept,
        dcat:Resource ;
    rdfs:label "Item I1413"@en-AU ;
    rdfs:comment "269 ZCA  Application to extend a review of anti dumping measures to include revocation - GraphNodeID: I1413"@en-AU ;
    skos:definition "269 ZCA  Application to extend a review of anti dumping measures to include revocation"@en-AU ;
    skos:narrower C1901A00006:1354 ;
    skos:prefLabel "Item I1413"@en-AU ;
    dcat:accessURL "https://www.legislation.gov.au/C1901A00006/2024-07-01/2024-07-01/text/original/epub/OEBPS/document_4/document_4.html#_Toc172628847"^^xsd:anyURI .

C1901A00006:1414 a legcons:Item,
        skos:Concept,
        dcat:Resource ;
    rdfs:label "Item I1414"@en-AU ;
    rdfs:comment "269 ZCB  Content and lodgment of application to extend a review of anti dumping measures to include revocation - GraphNodeID: I1414"@en-AU ;
    skos:definition "269 ZCB  Content and lodgment of application to extend a review of anti dumping measures to include revocation"@en-AU ;
    skos:narrower C1901A00006:1354 ;
    skos:prefLabel "Item I1414"@en-AU ;
    dcat:accessURL "https://www.legislation.gov.au/C1901A00006/2024-07-01/2024-07-01/text/original/epub/OEBPS/document_4/document_4.html#_Toc172628848"^^xsd:anyURI .

C1901A00006:1415 a legcons:Item,
        skos:Concept,
        dcat:Resource ;
    rdfs:label "Item I1415"@en-AU ;
    rdfs:comment "269 ZCC  Consideration of applications and requests for extensions of reviews - GraphNodeID: I1415"@en-AU ;
    skos:definition "269 ZCC  Consideration of applications and requests for extensions of reviews"@en-AU ;
    skos:narrower C1901A00006:1354 ;
    skos:prefLabel "Item I1415"@en-AU ;
    dcat:accessURL "https://www.legislation.gov.au/C1901A00006/2024-07-01/2024-07-01/text/original/epub/OEBPS/document_4/document_4.html#_Toc172628849"^^xsd:anyURI .

C1901A00006:1416 a legcons:Item,
        skos:Concept,
        dcat:Resource ;
    rdfs:label "Item I1416"@en-AU ;
    rdfs:comment "269 ZD  Statement of essential facts in relation to review of anti dumping measures - GraphNodeID: I1416"@en-AU ;
    skos:definition "269 ZD  Statement of essential facts in relation to review of anti dumping measures"@en-AU ;
    skos:narrower C1901A00006:1354 ;
    skos:prefLabel "Item I1416"@en-AU ;
    dcat:accessURL "https://www.legislation.gov.au/C1901A00006/2024-07-01/2024-07-01/text/original/epub/OEBPS/document_4/document_4.html#_Toc172628850"^^xsd:anyURI .

C1901A00006:1417 a legcons:Item,
        skos:Concept,
        dcat:Resource ;
    rdfs:label "Item I1417"@en-AU ;
    rdfs:comment "269 ZDA  Report on review of measures - GraphNodeID: I1417"@en-AU ;
    skos:definition "269 ZDA  Report on review of measures"@en-AU ;
    skos:narrower C1901A00006:1354 ;
    skos:prefLabel "Item I1417"@en-AU ;
    dcat:accessURL "https://www.legislation.gov.au/C1901A00006/2024-07-01/2024-07-01/text/original/epub/OEBPS/document_4/document_4.html#_Toc172628851"^^xsd:anyURI .

C1901A00006:1418 a legcons:Item,
        skos:Concept,
        dcat:Resource ;
    rdfs:label "Item I1418"@en-AU ;
    rdfs:comment "269 ZDB  Powers of the Minister in relation to review of anti dumping measures - GraphNodeID: I1418"@en-AU ;
    skos:definition "269 ZDB  Powers of the Minister in relation to review of anti dumping measures"@en-AU ;
    skos:narrower C1901A00006:1354 ;
    skos:prefLabel "Item I1418"@en-AU ;
    dcat:accessURL "https://www.legislation.gov.au/C1901A00006/2024-07-01/2024-07-01/text/original/epub/OEBPS/document_4/document_4.html#_Toc172628852"^^xsd:anyURI .

C1901A00006:1419 a legcons:Division,
        skos:Concept,
        dcat:Resource ;
    rdfs:label "Division D1419"@en-AU ;
    rdfs:comment "Division 5 AAnti circumvention inquiries - GraphNodeID: D1419"@en-AU ;
    skos:definition "Division 5 AAnti circumvention inquiries"@en-AU ;
    skos:narrower C1901A00006:1327 ;
    skos:prefLabel "Division D1419"@en-AU ;
    dcat:accessURL "https://www.legislation.gov.au/C1901A00006/2024-07-01/2024-07-01/text/original/epub/OEBPS/document_4/document_4.html#_Toc172628853"^^xsd:anyURI .

C1901A00006:142 a legcons:Item,
        skos:Concept,
        dcat:Resource ;
    rdfs:label "Item I142"@en-AU ;
    rdfs:comment "71 AAAN  Cancellation of authority to deal with specified low value goods - GraphNodeID: I142"@en-AU ;
    skos:definition "71 AAAN  Cancellation of authority to deal with specified low value goods"@en-AU ;
    skos:narrower C1901A00006:131 ;
    skos:prefLabel "Item I142"@en-AU ;
    dcat:accessURL "https://www.legislation.gov.au/C1901A00006/2024-07-01/2024-07-01/text/original/epub/OEBPS/document_1/document_1.html#_Toc172623116"^^xsd:anyURI .

C1901A00006:1420 a legcons:Item,
        skos:Concept,
        dcat:Resource ;
    rdfs:label "Item I1420"@en-AU ;
    rdfs:comment "269 ZDBA  What this Division is about - GraphNodeID: I1420"@en-AU ;
    skos:definition "269 ZDBA  What this Division is about"@en-AU ;
    skos:narrower C1901A00006:1354 ;
    skos:prefLabel "Item I1420"@en-AU ;
    dcat:accessURL "https://www.legislation.gov.au/C1901A00006/2024-07-01/2024-07-01/text/original/epub/OEBPS/document_4/document_4.html#_Toc172628854"^^xsd:anyURI .

C1901A00006:1421 a legcons:Item,
        skos:Concept,
        dcat:Resource ;
    rdfs:label "Item I1421"@en-AU ;
    rdfs:comment "269 ZDBB  Circumvention activities - GraphNodeID: I1421"@en-AU ;
    skos:definition "269 ZDBB  Circumvention activities"@en-AU ;
    skos:narrower C1901A00006:1354 ;
    skos:prefLabel "Item I1421"@en-AU ;
    dcat:accessURL "https://www.legislation.gov.au/C1901A00006/2024-07-01/2024-07-01/text/original/epub/OEBPS/document_4/document_4.html#_Toc172628855"^^xsd:anyURI .

C1901A00006:1422 a legcons:Item,
        skos:Concept,
        dcat:Resource ;
    rdfs:label "Item I1422"@en-AU ;
    rdfs:comment "269 ZDBC  Applications and requests for conduct of an anti circumvention inquiry - GraphNodeID: I1422"@en-AU ;
    skos:definition "269 ZDBC  Applications and requests for conduct of an anti circumvention inquiry"@en-AU ;
    skos:narrower C1901A00006:1354 ;
    skos:prefLabel "Item I1422"@en-AU ;
    dcat:accessURL "https://www.legislation.gov.au/C1901A00006/2024-07-01/2024-07-01/text/original/epub/OEBPS/document_4/document_4.html#_Toc172628856"^^xsd:anyURI .

C1901A00006:1423 a legcons:Item,
        skos:Concept,
        dcat:Resource ;
    rdfs:label "Item I1423"@en-AU ;
    rdfs:comment "269 ZDBD  Content and lodgement of applications for conduct of an anti circumvention inquiry - GraphNodeID: I1423"@en-AU ;
    skos:definition "269 ZDBD  Content and lodgement of applications for conduct of an anti circumvention inquiry"@en-AU ;
    skos:narrower C1901A00006:1354 ;
    skos:prefLabel "Item I1423"@en-AU ;
    dcat:accessURL "https://www.legislation.gov.au/C1901A00006/2024-07-01/2024-07-01/text/original/epub/OEBPS/document_4/document_4.html#_Toc172628857"^^xsd:anyURI .

C1901A00006:1424 a legcons:Item,
        skos:Concept,
        dcat:Resource ;
    rdfs:label "Item I1424"@en-AU ;
    rdfs:comment "269 ZDBE  Consideration of applications and requests for conduct of an anti circumvention inquiry - GraphNodeID: I1424"@en-AU ;
    skos:definition "269 ZDBE  Consideration of applications and requests for conduct of an anti circumvention inquiry"@en-AU ;
    skos:narrower C1901A00006:1354 ;
    skos:prefLabel "Item I1424"@en-AU ;
    dcat:accessURL "https://www.legislation.gov.au/C1901A00006/2024-07-01/2024-07-01/text/original/epub/OEBPS/document_4/document_4.html#_Toc172628858"^^xsd:anyURI .

C1901A00006:1425 a legcons:Item,
        skos:Concept,
        dcat:Resource ;
    rdfs:label "Item I1425"@en-AU ;
    rdfs:comment "269 ZDBEA  Termination of anti circumvention inquiry - GraphNodeID: I1425"@en-AU ;
    skos:definition "269 ZDBEA  Termination of anti circumvention inquiry"@en-AU ;
    skos:narrower C1901A00006:1354 ;
    skos:prefLabel "Item I1425"@en-AU ;
    dcat:accessURL "https://www.legislation.gov.au/C1901A00006/2024-07-01/2024-07-01/text/original/epub/OEBPS/document_4/document_4.html#_Toc172628859"^^xsd:anyURI .

C1901A00006:1426 a legcons:Item,
        skos:Concept,
        dcat:Resource ;
    rdfs:label "Item I1426"@en-AU ;
    rdfs:comment "269 ZDBF  Statement of essential facts in relation to conduct of an anti circumvention inquiry - GraphNodeID: I1426"@en-AU ;
    skos:definition "269 ZDBF  Statement of essential facts in relation to conduct of an anti circumvention inquiry"@en-AU ;
    skos:narrower C1901A00006:1354 ;
    skos:prefLabel "Item I1426"@en-AU ;
    dcat:accessURL "https://www.legislation.gov.au/C1901A00006/2024-07-01/2024-07-01/text/original/epub/OEBPS/document_4/document_4.html#_Toc172628860"^^xsd:anyURI .

C1901A00006:1427 a legcons:Item,
        skos:Concept,
        dcat:Resource ;
    rdfs:label "Item I1427"@en-AU ;
    rdfs:comment "269 ZDBG  Report on anti circumvention inquiry - GraphNodeID: I1427"@en-AU ;
    skos:definition "269 ZDBG  Report on anti circumvention inquiry"@en-AU ;
    skos:narrower C1901A00006:1354 ;
    skos:prefLabel "Item I1427"@en-AU ;
    dcat:accessURL "https://www.legislation.gov.au/C1901A00006/2024-07-01/2024-07-01/text/original/epub/OEBPS/document_4/document_4.html#_Toc172628861"^^xsd:anyURI .

C1901A00006:1428 a legcons:Item,
        skos:Concept,
        dcat:Resource ;
    rdfs:label "Item I1428"@en-AU ;
    rdfs:comment "269 ZDBH  Ministers powers in relation to anti circumvention inquiry - GraphNodeID: I1428"@en-AU ;
    skos:definition "269 ZDBH  Ministers powers in relation to anti circumvention inquiry"@en-AU ;
    skos:narrower C1901A00006:1354 ;
    skos:prefLabel "Item I1428"@en-AU ;
    dcat:accessURL "https://www.legislation.gov.au/C1901A00006/2024-07-01/2024-07-01/text/original/epub/OEBPS/document_4/document_4.html#_Toc172628862"^^xsd:anyURI .

C1901A00006:1429 a legcons:Division,
        skos:Concept,
        dcat:Resource ;
    rdfs:label "Division D1429"@en-AU ;
    rdfs:comment "Division 6 Certain exporters may seek accelerated review of dumping duty notices or countervailing duty notices - GraphNodeID: D1429"@en-AU ;
    skos:definition "Division 6 Certain exporters may seek accelerated review of dumping duty notices or countervailing duty notices"@en-AU ;
    skos:narrower C1901A00006:1327 ;
    skos:prefLabel "Division D1429"@en-AU ;
    dcat:accessURL "https://www.legislation.gov.au/C1901A00006/2024-07-01/2024-07-01/text/original/epub/OEBPS/document_4/document_4.html#_Toc172628863"^^xsd:anyURI .

C1901A00006:143 a legcons:Item,
        skos:Concept,
        dcat:Resource ;
    rdfs:label "Item I143"@en-AU ;
    rdfs:comment "71 AAAO  Officer may seek further information in relation to self assessed clearance declaration - GraphNodeID: I143"@en-AU ;
    skos:definition "71 AAAO  Officer may seek further information in relation to self assessed clearance declaration"@en-AU ;
    skos:narrower C1901A00006:131 ;
    skos:prefLabel "Item I143"@en-AU ;
    dcat:accessURL "https://www.legislation.gov.au/C1901A00006/2024-07-01/2024-07-01/text/original/epub/OEBPS/document_1/document_1.html#_Toc172623117"^^xsd:anyURI .

C1901A00006:1430 a legcons:Item,
        skos:Concept,
        dcat:Resource ;
    rdfs:label "Item I1430"@en-AU ;
    rdfs:comment "269 ZDC  What this Division is about - GraphNodeID: I1430"@en-AU ;
    skos:definition "269 ZDC  What this Division is about"@en-AU ;
    skos:narrower C1901A00006:1354 ;
    skos:prefLabel "Item I1430"@en-AU ;
    dcat:accessURL "https://www.legislation.gov.au/C1901A00006/2024-07-01/2024-07-01/text/original/epub/OEBPS/document_4/document_4.html#_Toc172628864"^^xsd:anyURI .

C1901A00006:1431 a legcons:Item,
        skos:Concept,
        dcat:Resource ;
    rdfs:label "Item I1431"@en-AU ;
    rdfs:comment "269 ZE  Circumstances in which accelerated review may be sought - GraphNodeID: I1431"@en-AU ;
    skos:definition "269 ZE  Circumstances in which accelerated review may be sought"@en-AU ;
    skos:narrower C1901A00006:1354 ;
    skos:prefLabel "Item I1431"@en-AU ;
    dcat:accessURL "https://www.legislation.gov.au/C1901A00006/2024-07-01/2024-07-01/text/original/epub/OEBPS/document_4/document_4.html#_Toc172628865"^^xsd:anyURI .

C1901A00006:1432 a legcons:Item,
        skos:Concept,
        dcat:Resource ;
    rdfs:label "Item I1432"@en-AU ;
    rdfs:comment "269 ZF  Application for accelerated review - GraphNodeID: I1432"@en-AU ;
    skos:definition "269 ZF  Application for accelerated review"@en-AU ;
    skos:narrower C1901A00006:1354 ;
    skos:prefLabel "Item I1432"@en-AU ;
    dcat:accessURL "https://www.legislation.gov.au/C1901A00006/2024-07-01/2024-07-01/text/original/epub/OEBPS/document_4/document_4.html#_Toc172628866"^^xsd:anyURI .

C1901A00006:1433 a legcons:Item,
        skos:Concept,
        dcat:Resource ;
    rdfs:label "Item I1433"@en-AU ;
    rdfs:comment "269 ZG  Consideration of application - GraphNodeID: I1433"@en-AU ;
    skos:definition "269 ZG  Consideration of application"@en-AU ;
    skos:narrower C1901A00006:1354 ;
    skos:prefLabel "Item I1433"@en-AU ;
    dcat:accessURL "https://www.legislation.gov.au/C1901A00006/2024-07-01/2024-07-01/text/original/epub/OEBPS/document_4/document_4.html#_Toc172628867"^^xsd:anyURI .

C1901A00006:1434 a legcons:Item,
        skos:Concept,
        dcat:Resource ;
    rdfs:label "Item I1434"@en-AU ;
    rdfs:comment "269 ZH  Effect of accelerated review - GraphNodeID: I1434"@en-AU ;
    skos:definition "269 ZH  Effect of accelerated review"@en-AU ;
    skos:narrower C1901A00006:1354 ;
    skos:prefLabel "Item I1434"@en-AU ;
    dcat:accessURL "https://www.legislation.gov.au/C1901A00006/2024-07-01/2024-07-01/text/original/epub/OEBPS/document_4/document_4.html#_Toc172628868"^^xsd:anyURI .

C1901A00006:1435 a legcons:Division,
        skos:Concept,
        dcat:Resource ;
    rdfs:label "Division D1435"@en-AU ;
    rdfs:comment "Division 6 AContinuation of anti dumping measures - GraphNodeID: D1435"@en-AU ;
    skos:definition "Division 6 AContinuation of anti dumping measures"@en-AU ;
    skos:narrower C1901A00006:1327 ;
    skos:prefLabel "Division D1435"@en-AU ;
    dcat:accessURL "https://www.legislation.gov.au/C1901A00006/2024-07-01/2024-07-01/text/original/epub/OEBPS/document_4/document_4.html#_Toc172628869"^^xsd:anyURI .

C1901A00006:1436 a legcons:Item,
        skos:Concept,
        dcat:Resource ;
    rdfs:label "Item I1436"@en-AU ;
    rdfs:comment "269 ZHA  What this Division is about - GraphNodeID: I1436"@en-AU ;
    skos:definition "269 ZHA  What this Division is about"@en-AU ;
    skos:narrower C1901A00006:1354 ;
    skos:prefLabel "Item I1436"@en-AU ;
    dcat:accessURL "https://www.legislation.gov.au/C1901A00006/2024-07-01/2024-07-01/text/original/epub/OEBPS/document_4/document_4.html#_Toc172628870"^^xsd:anyURI .

C1901A00006:1437 a legcons:Item,
        skos:Concept,
        dcat:Resource ;
    rdfs:label "Item I1437"@en-AU ;
    rdfs:comment "269 ZHB  Applications for continuation of anti dumping measures - GraphNodeID: I1437"@en-AU ;
    skos:definition "269 ZHB  Applications for continuation of anti dumping measures"@en-AU ;
    skos:narrower C1901A00006:1354 ;
    skos:prefLabel "Item I1437"@en-AU ;
    dcat:accessURL "https://www.legislation.gov.au/C1901A00006/2024-07-01/2024-07-01/text/original/epub/OEBPS/document_4/document_4.html#_Toc172628871"^^xsd:anyURI .

C1901A00006:1438 a legcons:Item,
        skos:Concept,
        dcat:Resource ;
    rdfs:label "Item I1438"@en-AU ;
    rdfs:comment "269 ZHC  Content and lodgment of application for continuation of anti dumping measures - GraphNodeID: I1438"@en-AU ;
    skos:definition "269 ZHC  Content and lodgment of application for continuation of anti dumping measures"@en-AU ;
    skos:narrower C1901A00006:1354 ;
    skos:prefLabel "Item I1438"@en-AU ;
    dcat:accessURL "https://www.legislation.gov.au/C1901A00006/2024-07-01/2024-07-01/text/original/epub/OEBPS/document_4/document_4.html#_Toc172628872"^^xsd:anyURI .

C1901A00006:1439 a legcons:Item,
        skos:Concept,
        dcat:Resource ;
    rdfs:label "Item I1439"@en-AU ;
    rdfs:comment "269 ZHD  Consideration of applications for continuation of anti dumping measures - GraphNodeID: I1439"@en-AU ;
    skos:definition "269 ZHD  Consideration of applications for continuation of anti dumping measures"@en-AU ;
    skos:narrower C1901A00006:1354 ;
    skos:prefLabel "Item I1439"@en-AU ;
    dcat:accessURL "https://www.legislation.gov.au/C1901A00006/2024-07-01/2024-07-01/text/original/epub/OEBPS/document_4/document_4.html#_Toc172628873"^^xsd:anyURI .

C1901A00006:144 a legcons:Item,
        skos:Concept,
        dcat:Resource ;
    rdfs:label "Item I144"@en-AU ;
    rdfs:comment "71 AAAP  Withdrawal of self assessed clearance declarations - GraphNodeID: I144"@en-AU ;
    skos:definition "71 AAAP  Withdrawal of self assessed clearance declarations"@en-AU ;
    skos:narrower C1901A00006:131 ;
    skos:prefLabel "Item I144"@en-AU ;
    dcat:accessURL "https://www.legislation.gov.au/C1901A00006/2024-07-01/2024-07-01/text/original/epub/OEBPS/document_1/document_1.html#_Toc172623118"^^xsd:anyURI .

C1901A00006:1440 a legcons:Item,
        skos:Concept,
        dcat:Resource ;
    rdfs:label "Item I1440"@en-AU ;
    rdfs:comment "269 ZHE  Statement of essential facts in relation to continuation of anti dumping measures - GraphNodeID: I1440"@en-AU ;
    skos:definition "269 ZHE  Statement of essential facts in relation to continuation of anti dumping measures"@en-AU ;
    skos:narrower C1901A00006:1354 ;
    skos:prefLabel "Item I1440"@en-AU ;
    dcat:accessURL "https://www.legislation.gov.au/C1901A00006/2024-07-01/2024-07-01/text/original/epub/OEBPS/document_4/document_4.html#_Toc172628874"^^xsd:anyURI .

C1901A00006:1441 a legcons:Item,
        skos:Concept,
        dcat:Resource ;
    rdfs:label "Item I1441"@en-AU ;
    rdfs:comment "269 ZHF  Report on application for continuation of anti dumping measures - GraphNodeID: I1441"@en-AU ;
    skos:definition "269 ZHF  Report on application for continuation of anti dumping measures"@en-AU ;
    skos:narrower C1901A00006:1354 ;
    skos:prefLabel "Item I1441"@en-AU ;
    dcat:accessURL "https://www.legislation.gov.au/C1901A00006/2024-07-01/2024-07-01/text/original/epub/OEBPS/document_4/document_4.html#_Toc172628875"^^xsd:anyURI .

C1901A00006:1442 a legcons:Item,
        skos:Concept,
        dcat:Resource ;
    rdfs:label "Item I1442"@en-AU ;
    rdfs:comment "269 ZHG  Powers of the Minister in relation to continuation of anti dumping measures - GraphNodeID: I1442"@en-AU ;
    skos:definition "269 ZHG  Powers of the Minister in relation to continuation of anti dumping measures"@en-AU ;
    skos:narrower C1901A00006:1354 ;
    skos:prefLabel "Item I1442"@en-AU ;
    dcat:accessURL "https://www.legislation.gov.au/C1901A00006/2024-07-01/2024-07-01/text/original/epub/OEBPS/document_4/document_4.html#_Toc172628876"^^xsd:anyURI .

C1901A00006:1443 a legcons:Division,
        skos:Concept,
        dcat:Resource ;
    rdfs:label "Division D1443"@en-AU ;
    rdfs:comment "Division 7 Procedural and evidentiary matters - GraphNodeID: D1443"@en-AU ;
    skos:definition "Division 7 Procedural and evidentiary matters"@en-AU ;
    skos:narrower C1901A00006:1327 ;
    skos:prefLabel "Division D1443"@en-AU ;
    dcat:accessURL "https://www.legislation.gov.au/C1901A00006/2024-07-01/2024-07-01/text/original/epub/OEBPS/document_4/document_4.html#_Toc172628877"^^xsd:anyURI .

C1901A00006:1444 a legcons:Item,
        skos:Concept,
        dcat:Resource ;
    rdfs:label "Item I1444"@en-AU ;
    rdfs:comment "269 ZHH  What this Division is about - GraphNodeID: I1444"@en-AU ;
    skos:definition "269 ZHH  What this Division is about"@en-AU ;
    skos:narrower C1901A00006:1354 ;
    skos:prefLabel "Item I1444"@en-AU ;
    dcat:accessURL "https://www.legislation.gov.au/C1901A00006/2024-07-01/2024-07-01/text/original/epub/OEBPS/document_4/document_4.html#_Toc172628878"^^xsd:anyURI .

C1901A00006:1445 a legcons:Item,
        skos:Concept,
        dcat:Resource ;
    rdfs:label "Item I1445"@en-AU ;
    rdfs:comment "269 ZHI  Minister may extend certain periods of time - GraphNodeID: I1445"@en-AU ;
    skos:definition "269 ZHI  Minister may extend certain periods of time"@en-AU ;
    skos:narrower C1901A00006:1354 ;
    skos:prefLabel "Item I1445"@en-AU ;
    dcat:accessURL "https://www.legislation.gov.au/C1901A00006/2024-07-01/2024-07-01/text/original/epub/OEBPS/document_4/document_4.html#_Toc172628879"^^xsd:anyURI .

C1901A00006:1446 a legcons:Item,
        skos:Concept,
        dcat:Resource ;
    rdfs:label "Item I1446"@en-AU ;
    rdfs:comment "269 ZI  Public notice - GraphNodeID: I1446"@en-AU ;
    skos:definition "269 ZI  Public notice"@en-AU ;
    skos:narrower C1901A00006:1354 ;
    skos:prefLabel "Item I1446"@en-AU ;
    dcat:accessURL "https://www.legislation.gov.au/C1901A00006/2024-07-01/2024-07-01/text/original/epub/OEBPS/document_4/document_4.html#_Toc172628880"^^xsd:anyURI .

C1901A00006:1447 a legcons:Item,
        skos:Concept,
        dcat:Resource ;
    rdfs:label "Item I1447"@en-AU ;
    rdfs:comment "269 ZJ  Commissioner to maintain public record for certain purposes - GraphNodeID: I1447"@en-AU ;
    skos:definition "269 ZJ  Commissioner to maintain public record for certain purposes"@en-AU ;
    skos:narrower C1901A00006:1354 ;
    skos:prefLabel "Item I1447"@en-AU ;
    dcat:accessURL "https://www.legislation.gov.au/C1901A00006/2024-07-01/2024-07-01/text/original/epub/OEBPS/document_4/document_4.html#_Toc172628881"^^xsd:anyURI .

C1901A00006:1448 a legcons:Division,
        skos:Concept,
        dcat:Resource ;
    rdfs:label "Division D1448"@en-AU ;
    rdfs:comment "Division 8 Review Panel - GraphNodeID: D1448"@en-AU ;
    skos:definition "Division 8 Review Panel"@en-AU ;
    skos:narrower C1901A00006:1327 ;
    skos:prefLabel "Division D1448"@en-AU ;
    dcat:accessURL "https://www.legislation.gov.au/C1901A00006/2024-07-01/2024-07-01/text/original/epub/OEBPS/document_4/document_4.html#_Toc172628882"^^xsd:anyURI .

C1901A00006:1449 a legcons:Item,
        skos:Concept,
        dcat:Resource ;
    rdfs:label "Item I1449"@en-AU ;
    rdfs:comment "269 ZK  What this Division is about - GraphNodeID: I1449"@en-AU ;
    skos:definition "269 ZK  What this Division is about"@en-AU ;
    skos:narrower C1901A00006:1354 ;
    skos:prefLabel "Item I1449"@en-AU ;
    dcat:accessURL "https://www.legislation.gov.au/C1901A00006/2024-07-01/2024-07-01/text/original/epub/OEBPS/document_4/document_4.html#_Toc172628883"^^xsd:anyURI .

C1901A00006:145 a legcons:Item,
        skos:Concept,
        dcat:Resource ;
    rdfs:label "Item I145"@en-AU ;
    rdfs:comment "71 AAAQ  Further self assessed clearance declaration not to be given while there is an existing self assessed clearance declaration - GraphNodeID: I145"@en-AU ;
    skos:definition "71 AAAQ  Further self assessed clearance declaration not to be given while there is an existing self assessed clearance declaration"@en-AU ;
    skos:narrower C1901A00006:131 ;
    skos:prefLabel "Item I145"@en-AU ;
    dcat:accessURL "https://www.legislation.gov.au/C1901A00006/2024-07-01/2024-07-01/text/original/epub/OEBPS/document_1/document_1.html#_Toc172623119"^^xsd:anyURI .

C1901A00006:1450 a legcons:Item,
        skos:Concept,
        dcat:Resource ;
    rdfs:label "Item I1450"@en-AU ;
    rdfs:comment "269 ZL  Establishment of Review Panel - GraphNodeID: I1450"@en-AU ;
    skos:definition "269 ZL  Establishment of Review Panel"@en-AU ;
    skos:narrower C1901A00006:1354 ;
    skos:prefLabel "Item I1450"@en-AU ;
    dcat:accessURL "https://www.legislation.gov.au/C1901A00006/2024-07-01/2024-07-01/text/original/epub/OEBPS/document_4/document_4.html#_Toc172628884"^^xsd:anyURI .

C1901A00006:1451 a legcons:Item,
        skos:Concept,
        dcat:Resource ;
    rdfs:label "Item I1451"@en-AU ;
    rdfs:comment "269 ZM  Membership of the Review Panel - GraphNodeID: I1451"@en-AU ;
    skos:definition "269 ZM  Membership of the Review Panel"@en-AU ;
    skos:narrower C1901A00006:1354 ;
    skos:prefLabel "Item I1451"@en-AU ;
    dcat:accessURL "https://www.legislation.gov.au/C1901A00006/2024-07-01/2024-07-01/text/original/epub/OEBPS/document_4/document_4.html#_Toc172628885"^^xsd:anyURI .

C1901A00006:1452 a legcons:Item,
        skos:Concept,
        dcat:Resource ;
    rdfs:label "Item I1452"@en-AU ;
    rdfs:comment "269 ZN  Review Panels powers - GraphNodeID: I1452"@en-AU ;
    skos:definition "269 ZN  Review Panels powers"@en-AU ;
    skos:narrower C1901A00006:1354 ;
    skos:prefLabel "Item I1452"@en-AU ;
    dcat:accessURL "https://www.legislation.gov.au/C1901A00006/2024-07-01/2024-07-01/text/original/epub/OEBPS/document_4/document_4.html#_Toc172628886"^^xsd:anyURI .

C1901A00006:1453 a legcons:Item,
        skos:Concept,
        dcat:Resource ;
    rdfs:label "Item I1453"@en-AU ;
    rdfs:comment "269 ZO  Protection of members - GraphNodeID: I1453"@en-AU ;
    skos:definition "269 ZO  Protection of members"@en-AU ;
    skos:narrower C1901A00006:1354 ;
    skos:prefLabel "Item I1453"@en-AU ;
    dcat:accessURL "https://www.legislation.gov.au/C1901A00006/2024-07-01/2024-07-01/text/original/epub/OEBPS/document_4/document_4.html#_Toc172628887"^^xsd:anyURI .

C1901A00006:1454 a legcons:Item,
        skos:Concept,
        dcat:Resource ;
    rdfs:label "Item I1454"@en-AU ;
    rdfs:comment "269 ZP  Appointment of members - GraphNodeID: I1454"@en-AU ;
    skos:definition "269 ZP  Appointment of members"@en-AU ;
    skos:narrower C1901A00006:1354 ;
    skos:prefLabel "Item I1454"@en-AU ;
    dcat:accessURL "https://www.legislation.gov.au/C1901A00006/2024-07-01/2024-07-01/text/original/epub/OEBPS/document_4/document_4.html#_Toc172628888"^^xsd:anyURI .

C1901A00006:1455 a legcons:Item,
        skos:Concept,
        dcat:Resource ;
    rdfs:label "Item I1455"@en-AU ;
    rdfs:comment "269 ZQ  Period of appointment for members - GraphNodeID: I1455"@en-AU ;
    skos:definition "269 ZQ  Period of appointment for members"@en-AU ;
    skos:narrower C1901A00006:1354 ;
    skos:prefLabel "Item I1455"@en-AU ;
    dcat:accessURL "https://www.legislation.gov.au/C1901A00006/2024-07-01/2024-07-01/text/original/epub/OEBPS/document_4/document_4.html#_Toc172628889"^^xsd:anyURI .

C1901A00006:1456 a legcons:Item,
        skos:Concept,
        dcat:Resource ;
    rdfs:label "Item I1456"@en-AU ;
    rdfs:comment "269 ZR  Terms and conditions of appointment - GraphNodeID: I1456"@en-AU ;
    skos:definition "269 ZR  Terms and conditions of appointment"@en-AU ;
    skos:narrower C1901A00006:1354 ;
    skos:prefLabel "Item I1456"@en-AU ;
    dcat:accessURL "https://www.legislation.gov.au/C1901A00006/2024-07-01/2024-07-01/text/original/epub/OEBPS/document_4/document_4.html#_Toc172628890"^^xsd:anyURI .

C1901A00006:1457 a legcons:Item,
        skos:Concept,
        dcat:Resource ;
    rdfs:label "Item I1457"@en-AU ;
    rdfs:comment "269 ZS  Disclosure of interests to the Minister - GraphNodeID: I1457"@en-AU ;
    skos:definition "269 ZS  Disclosure of interests to the Minister"@en-AU ;
    skos:narrower C1901A00006:1354 ;
    skos:prefLabel "Item I1457"@en-AU ;
    dcat:accessURL "https://www.legislation.gov.au/C1901A00006/2024-07-01/2024-07-01/text/original/epub/OEBPS/document_4/document_4.html#_Toc172628891"^^xsd:anyURI .

C1901A00006:1458 a legcons:Item,
        skos:Concept,
        dcat:Resource ;
    rdfs:label "Item I1458"@en-AU ;
    rdfs:comment "269 ZT  Outside employment - GraphNodeID: I1458"@en-AU ;
    skos:definition "269 ZT  Outside employment"@en-AU ;
    skos:narrower C1901A00006:1354 ;
    skos:prefLabel "Item I1458"@en-AU ;
    dcat:accessURL "https://www.legislation.gov.au/C1901A00006/2024-07-01/2024-07-01/text/original/epub/OEBPS/document_4/document_4.html#_Toc172628892"^^xsd:anyURI .

C1901A00006:1459 a legcons:Item,
        skos:Concept,
        dcat:Resource ;
    rdfs:label "Item I1459"@en-AU ;
    rdfs:comment "269 ZTA  Resignation - GraphNodeID: I1459"@en-AU ;
    skos:definition "269 ZTA  Resignation"@en-AU ;
    skos:narrower C1901A00006:1354 ;
    skos:prefLabel "Item I1459"@en-AU ;
    dcat:accessURL "https://www.legislation.gov.au/C1901A00006/2024-07-01/2024-07-01/text/original/epub/OEBPS/document_4/document_4.html#_Toc172628893"^^xsd:anyURI .

C1901A00006:146 a legcons:Item,
        skos:Concept,
        dcat:Resource ;
    rdfs:label "Item I146"@en-AU ;
    rdfs:comment "71 AAAR  Effect of withdrawal of a self assessed clearance declaration - GraphNodeID: I146"@en-AU ;
    skos:definition "71 AAAR  Effect of withdrawal of a self assessed clearance declaration"@en-AU ;
    skos:narrower C1901A00006:131 ;
    skos:prefLabel "Item I146"@en-AU ;
    dcat:accessURL "https://www.legislation.gov.au/C1901A00006/2024-07-01/2024-07-01/text/original/epub/OEBPS/document_1/document_1.html#_Toc172623120"^^xsd:anyURI .

C1901A00006:1460 a legcons:Item,
        skos:Concept,
        dcat:Resource ;
    rdfs:label "Item I1460"@en-AU ;
    rdfs:comment "269 ZTB  Termination of appointment - GraphNodeID: I1460"@en-AU ;
    skos:definition "269 ZTB  Termination of appointment"@en-AU ;
    skos:narrower C1901A00006:1354 ;
    skos:prefLabel "Item I1460"@en-AU ;
    dcat:accessURL "https://www.legislation.gov.au/C1901A00006/2024-07-01/2024-07-01/text/original/epub/OEBPS/document_4/document_4.html#_Toc172628894"^^xsd:anyURI .

C1901A00006:1461 a legcons:Item,
        skos:Concept,
        dcat:Resource ;
    rdfs:label "Item I1461"@en-AU ;
    rdfs:comment "269 ZTC  Acting appointments - GraphNodeID: I1461"@en-AU ;
    skos:definition "269 ZTC  Acting appointments"@en-AU ;
    skos:narrower C1901A00006:1354 ;
    skos:prefLabel "Item I1461"@en-AU ;
    dcat:accessURL "https://www.legislation.gov.au/C1901A00006/2024-07-01/2024-07-01/text/original/epub/OEBPS/document_4/document_4.html#_Toc172628895"^^xsd:anyURI .

C1901A00006:1462 a legcons:Item,
        skos:Concept,
        dcat:Resource ;
    rdfs:label "Item I1462"@en-AU ;
    rdfs:comment "269 ZTD  Provision of resources to Review Panel - GraphNodeID: I1462"@en-AU ;
    skos:definition "269 ZTD  Provision of resources to Review Panel"@en-AU ;
    skos:narrower C1901A00006:1354 ;
    skos:prefLabel "Item I1462"@en-AU ;
    dcat:accessURL "https://www.legislation.gov.au/C1901A00006/2024-07-01/2024-07-01/text/original/epub/OEBPS/document_4/document_4.html#_Toc172628896"^^xsd:anyURI .

C1901A00006:1463 a legcons:Item,
        skos:Concept,
        dcat:Resource ;
    rdfs:label "Item I1463"@en-AU ;
    rdfs:comment "269 ZU  Review Panel may supply information - GraphNodeID: I1463"@en-AU ;
    skos:definition "269 ZU  Review Panel may supply information"@en-AU ;
    skos:narrower C1901A00006:1354 ;
    skos:prefLabel "Item I1463"@en-AU ;
    dcat:accessURL "https://www.legislation.gov.au/C1901A00006/2024-07-01/2024-07-01/text/original/epub/OEBPS/document_4/document_4.html#_Toc172628897"^^xsd:anyURI .

C1901A00006:1464 a legcons:Item,
        skos:Concept,
        dcat:Resource ;
    rdfs:label "Item I1464"@en-AU ;
    rdfs:comment "269 ZV  False or misleading information - GraphNodeID: I1464"@en-AU ;
    skos:definition "269 ZV  False or misleading information"@en-AU ;
    skos:narrower C1901A00006:1354 ;
    skos:prefLabel "Item I1464"@en-AU ;
    dcat:accessURL "https://www.legislation.gov.au/C1901A00006/2024-07-01/2024-07-01/text/original/epub/OEBPS/document_4/document_4.html#_Toc172628898"^^xsd:anyURI .

C1901A00006:1467 a legcons:Item,
        skos:Concept,
        dcat:Resource ;
    rdfs:label "Item I1467"@en-AU ;
    rdfs:comment "269 ZW  What this Division is about - GraphNodeID: I1467"@en-AU ;
    skos:definition "269 ZW  What this Division is about"@en-AU ;
    skos:narrower C1901A00006:1466 ;
    skos:prefLabel "Item I1467"@en-AU ;
    dcat:accessURL "https://www.legislation.gov.au/C1901A00006/2024-07-01/2024-07-01/text/original/epub/OEBPS/document_4/document_4.html#_Toc172628901"^^xsd:anyURI .

C1901A00006:1468 a legcons:Item,
        skos:Concept,
        dcat:Resource ;
    rdfs:label "Item I1468"@en-AU ;
    rdfs:comment "269 ZX  Definitions - GraphNodeID: I1468"@en-AU ;
    skos:definition "269 ZX  Definitions"@en-AU ;
    skos:narrower C1901A00006:1466 ;
    skos:prefLabel "Item I1468"@en-AU ;
    dcat:accessURL "https://www.legislation.gov.au/C1901A00006/2024-07-01/2024-07-01/text/original/epub/OEBPS/document_4/document_4.html#_Toc172628902"^^xsd:anyURI .

C1901A00006:1469 a legcons:Item,
        skos:Concept,
        dcat:Resource ;
    rdfs:label "Item I1469"@en-AU ;
    rdfs:comment "269 ZY  Form and manner of applications - GraphNodeID: I1469"@en-AU ;
    skos:definition "269 ZY  Form and manner of applications"@en-AU ;
    skos:narrower C1901A00006:1466 ;
    skos:prefLabel "Item I1469"@en-AU ;
    dcat:accessURL "https://www.legislation.gov.au/C1901A00006/2024-07-01/2024-07-01/text/original/epub/OEBPS/document_4/document_4.html#_Toc172628903"^^xsd:anyURI .

C1901A00006:147 a legcons:Item,
        skos:Concept,
        dcat:Resource ;
    rdfs:label "Item I147"@en-AU ;
    rdfs:comment "71 AAAS  Annotation of self assessed clearance declaration by Collector for certain purposes not to constitute withdrawal - GraphNodeID: I147"@en-AU ;
    skos:definition "71 AAAS  Annotation of self assessed clearance declaration by Collector for certain purposes not to constitute withdrawal"@en-AU ;
    skos:narrower C1901A00006:131 ;
    skos:prefLabel "Item I147"@en-AU ;
    dcat:accessURL "https://www.legislation.gov.au/C1901A00006/2024-07-01/2024-07-01/text/original/epub/OEBPS/document_1/document_1.html#_Toc172623121"^^xsd:anyURI .

C1901A00006:1470 a legcons:Item,
        skos:Concept,
        dcat:Resource ;
    rdfs:label "Item I1470"@en-AU ;
    rdfs:comment "269 ZYA  Constitution of Review Panel for purposes of review - GraphNodeID: I1470"@en-AU ;
    skos:definition "269 ZYA  Constitution of Review Panel for purposes of review"@en-AU ;
    skos:narrower C1901A00006:1466 ;
    skos:prefLabel "Item I1470"@en-AU ;
    dcat:accessURL "https://www.legislation.gov.au/C1901A00006/2024-07-01/2024-07-01/text/original/epub/OEBPS/document_4/document_4.html#_Toc172628904"^^xsd:anyURI .

C1901A00006:1471 a legcons:Item,
        skos:Concept,
        dcat:Resource ;
    rdfs:label "Item I1471"@en-AU ;
    rdfs:comment "269 ZYB  Member unavailable to complete review - GraphNodeID: I1471"@en-AU ;
    skos:definition "269 ZYB  Member unavailable to complete review"@en-AU ;
    skos:narrower C1901A00006:1466 ;
    skos:prefLabel "Item I1471"@en-AU ;
    dcat:accessURL "https://www.legislation.gov.au/C1901A00006/2024-07-01/2024-07-01/text/original/epub/OEBPS/document_4/document_4.html#_Toc172628905"^^xsd:anyURI .

C1901A00006:1472 a legcons:Item,
        skos:Concept,
        dcat:Resource ;
    rdfs:label "Item I1472"@en-AU ;
    rdfs:comment "269 ZZ  Review Panel to have regard to same considerations as Minister - GraphNodeID: I1472"@en-AU ;
    skos:definition "269 ZZ  Review Panel to have regard to same considerations as Minister"@en-AU ;
    skos:narrower C1901A00006:1466 ;
    skos:prefLabel "Item I1472"@en-AU ;
    dcat:accessURL "https://www.legislation.gov.au/C1901A00006/2024-07-01/2024-07-01/text/original/epub/OEBPS/document_4/document_4.html#_Toc172628906"^^xsd:anyURI .

C1901A00006:1474 a legcons:Item,
        skos:Concept,
        dcat:Resource ;
    rdfs:label "Item I1474"@en-AU ;
    rdfs:comment "269 ZZA  Reviewable decisions - GraphNodeID: I1474"@en-AU ;
    skos:definition "269 ZZA  Reviewable decisions"@en-AU ;
    skos:narrower C1901A00006:1473 ;
    skos:prefLabel "Item I1474"@en-AU ;
    dcat:accessURL "https://www.legislation.gov.au/C1901A00006/2024-07-01/2024-07-01/text/original/epub/OEBPS/document_4/document_4.html#_Toc172628908"^^xsd:anyURI .

C1901A00006:1475 a legcons:Item,
        skos:Concept,
        dcat:Resource ;
    rdfs:label "Item I1475"@en-AU ;
    rdfs:comment "269 ZZB  Overview of a review of Ministers decision - GraphNodeID: I1475"@en-AU ;
    skos:definition "269 ZZB  Overview of a review of Ministers decision"@en-AU ;
    skos:narrower C1901A00006:1473 ;
    skos:prefLabel "Item I1475"@en-AU ;
    dcat:accessURL "https://www.legislation.gov.au/C1901A00006/2024-07-01/2024-07-01/text/original/epub/OEBPS/document_4/document_4.html#_Toc172628909"^^xsd:anyURI .

C1901A00006:1476 a legcons:Item,
        skos:Concept,
        dcat:Resource ;
    rdfs:label "Item I1476"@en-AU ;
    rdfs:comment "269 ZZC  Who may seek a review - GraphNodeID: I1476"@en-AU ;
    skos:definition "269 ZZC  Who may seek a review"@en-AU ;
    skos:narrower C1901A00006:1473 ;
    skos:prefLabel "Item I1476"@en-AU ;
    dcat:accessURL "https://www.legislation.gov.au/C1901A00006/2024-07-01/2024-07-01/text/original/epub/OEBPS/document_4/document_4.html#_Toc172628910"^^xsd:anyURI .

C1901A00006:1477 a legcons:Item,
        skos:Concept,
        dcat:Resource ;
    rdfs:label "Item I1477"@en-AU ;
    rdfs:comment "269 ZZD  When must an application be made - GraphNodeID: I1477"@en-AU ;
    skos:definition "269 ZZD  When must an application be made"@en-AU ;
    skos:narrower C1901A00006:1473 ;
    skos:prefLabel "Item I1477"@en-AU ;
    dcat:accessURL "https://www.legislation.gov.au/C1901A00006/2024-07-01/2024-07-01/text/original/epub/OEBPS/document_4/document_4.html#_Toc172628911"^^xsd:anyURI .

C1901A00006:1478 a legcons:Item,
        skos:Concept,
        dcat:Resource ;
    rdfs:label "Item I1478"@en-AU ;
    rdfs:comment "269 ZZE  How must an application be made - GraphNodeID: I1478"@en-AU ;
    skos:definition "269 ZZE  How must an application be made"@en-AU ;
    skos:narrower C1901A00006:1473 ;
    skos:prefLabel "Item I1478"@en-AU ;
    dcat:accessURL "https://www.legislation.gov.au/C1901A00006/2024-07-01/2024-07-01/text/original/epub/OEBPS/document_4/document_4.html#_Toc172628912"^^xsd:anyURI .

C1901A00006:1479 a legcons:Item,
        skos:Concept,
        dcat:Resource ;
    rdfs:label "Item I1479"@en-AU ;
    rdfs:comment "269 ZZF  Withdrawal of application - GraphNodeID: I1479"@en-AU ;
    skos:definition "269 ZZF  Withdrawal of application"@en-AU ;
    skos:narrower C1901A00006:1473 ;
    skos:prefLabel "Item I1479"@en-AU ;
    dcat:accessURL "https://www.legislation.gov.au/C1901A00006/2024-07-01/2024-07-01/text/original/epub/OEBPS/document_4/document_4.html#_Toc172628913"^^xsd:anyURI .

C1901A00006:148 a legcons:Item,
        skos:Concept,
        dcat:Resource ;
    rdfs:label "Item I148"@en-AU ;
    rdfs:comment "71 AAAT  Manner and effect of communicating self assessed clearance declarations to Department - GraphNodeID: I148"@en-AU ;
    skos:definition "71 AAAT  Manner and effect of communicating self assessed clearance declarations to Department"@en-AU ;
    skos:narrower C1901A00006:131 ;
    skos:prefLabel "Item I148"@en-AU ;
    dcat:accessURL "https://www.legislation.gov.au/C1901A00006/2024-07-01/2024-07-01/text/original/epub/OEBPS/document_1/document_1.html#_Toc172623122"^^xsd:anyURI .

C1901A00006:1480 a legcons:Item,
        skos:Concept,
        dcat:Resource ;
    rdfs:label "Item I1480"@en-AU ;
    rdfs:comment "269 ZZG  Rejection of applicationfailure to establish decision not the correct or preferable decision etc - GraphNodeID: I1480"@en-AU ;
    skos:definition "269 ZZG  Rejection of applicationfailure to establish decision not the correct or preferable decision etc"@en-AU ;
    skos:narrower C1901A00006:1473 ;
    skos:prefLabel "Item I1480"@en-AU ;
    dcat:accessURL "https://www.legislation.gov.au/C1901A00006/2024-07-01/2024-07-01/text/original/epub/OEBPS/document_4/document_4.html#_Toc172628914"^^xsd:anyURI .

C1901A00006:1481 a legcons:Item,
        skos:Concept,
        dcat:Resource ;
    rdfs:label "Item I1481"@en-AU ;
    rdfs:comment "269 ZZH  Rejection of applicationfailure to provide summary of confidential information - GraphNodeID: I1481"@en-AU ;
    skos:definition "269 ZZH  Rejection of applicationfailure to provide summary of confidential information"@en-AU ;
    skos:narrower C1901A00006:1473 ;
    skos:prefLabel "Item I1481"@en-AU ;
    dcat:accessURL "https://www.legislation.gov.au/C1901A00006/2024-07-01/2024-07-01/text/original/epub/OEBPS/document_4/document_4.html#_Toc172628915"^^xsd:anyURI .

C1901A00006:1482 a legcons:Item,
        skos:Concept,
        dcat:Resource ;
    rdfs:label "Item I1482"@en-AU ;
    rdfs:comment "269 ZZHA  Review Panel may hold conferences - GraphNodeID: I1482"@en-AU ;
    skos:definition "269 ZZHA  Review Panel may hold conferences"@en-AU ;
    skos:narrower C1901A00006:1473 ;
    skos:prefLabel "Item I1482"@en-AU ;
    dcat:accessURL "https://www.legislation.gov.au/C1901A00006/2024-07-01/2024-07-01/text/original/epub/OEBPS/document_4/document_4.html#_Toc172628916"^^xsd:anyURI .

C1901A00006:1483 a legcons:Item,
        skos:Concept,
        dcat:Resource ;
    rdfs:label "Item I1483"@en-AU ;
    rdfs:comment "269 ZZI  Public notification of review - GraphNodeID: I1483"@en-AU ;
    skos:definition "269 ZZI  Public notification of review"@en-AU ;
    skos:narrower C1901A00006:1473 ;
    skos:prefLabel "Item I1483"@en-AU ;
    dcat:accessURL "https://www.legislation.gov.au/C1901A00006/2024-07-01/2024-07-01/text/original/epub/OEBPS/document_4/document_4.html#_Toc172628917"^^xsd:anyURI .

C1901A00006:1484 a legcons:Item,
        skos:Concept,
        dcat:Resource ;
    rdfs:label "Item I1484"@en-AU ;
    rdfs:comment "269 ZZJ  Submissions in relation to reviewable decision - GraphNodeID: I1484"@en-AU ;
    skos:definition "269 ZZJ  Submissions in relation to reviewable decision"@en-AU ;
    skos:narrower C1901A00006:1473 ;
    skos:prefLabel "Item I1484"@en-AU ;
    dcat:accessURL "https://www.legislation.gov.au/C1901A00006/2024-07-01/2024-07-01/text/original/epub/OEBPS/document_4/document_4.html#_Toc172628918"^^xsd:anyURI .

C1901A00006:1485 a legcons:Item,
        skos:Concept,
        dcat:Resource ;
    rdfs:label "Item I1485"@en-AU ;
    rdfs:comment "269 ZZK  The review - GraphNodeID: I1485"@en-AU ;
    skos:definition "269 ZZK  The review"@en-AU ;
    skos:narrower C1901A00006:1473 ;
    skos:prefLabel "Item I1485"@en-AU ;
    dcat:accessURL "https://www.legislation.gov.au/C1901A00006/2024-07-01/2024-07-01/text/original/epub/OEBPS/document_4/document_4.html#_Toc172628919"^^xsd:anyURI .

C1901A00006:1486 a legcons:Item,
        skos:Concept,
        dcat:Resource ;
    rdfs:label "Item I1486"@en-AU ;
    rdfs:comment "269 ZZL  Review Panel may require reinvestigation by Commissioner before making recommendation to Minister - GraphNodeID: I1486"@en-AU ;
    skos:definition "269 ZZL  Review Panel may require reinvestigation by Commissioner before making recommendation to Minister"@en-AU ;
    skos:narrower C1901A00006:1473 ;
    skos:prefLabel "Item I1486"@en-AU ;
    dcat:accessURL "https://www.legislation.gov.au/C1901A00006/2024-07-01/2024-07-01/text/original/epub/OEBPS/document_4/document_4.html#_Toc172628920"^^xsd:anyURI .

C1901A00006:1487 a legcons:Item,
        skos:Concept,
        dcat:Resource ;
    rdfs:label "Item I1487"@en-AU ;
    rdfs:comment "269 ZZM  Ministers decision - GraphNodeID: I1487"@en-AU ;
    skos:definition "269 ZZM  Ministers decision"@en-AU ;
    skos:narrower C1901A00006:1473 ;
    skos:prefLabel "Item I1487"@en-AU ;
    dcat:accessURL "https://www.legislation.gov.au/C1901A00006/2024-07-01/2024-07-01/text/original/epub/OEBPS/document_4/document_4.html#_Toc172628921"^^xsd:anyURI .

C1901A00006:1489 a legcons:Item,
        skos:Concept,
        dcat:Resource ;
    rdfs:label "Item I1489"@en-AU ;
    rdfs:comment "269 ZZN  Reviewable decisions - GraphNodeID: I1489"@en-AU ;
    skos:definition "269 ZZN  Reviewable decisions"@en-AU ;
    skos:narrower C1901A00006:1488 ;
    skos:prefLabel "Item I1489"@en-AU ;
    dcat:accessURL "https://www.legislation.gov.au/C1901A00006/2024-07-01/2024-07-01/text/original/epub/OEBPS/document_4/document_4.html#_Toc172628923"^^xsd:anyURI .

C1901A00006:1490 a legcons:Item,
        skos:Concept,
        dcat:Resource ;
    rdfs:label "Item I1490"@en-AU ;
    rdfs:comment "269 ZZO  Who may seek a review - GraphNodeID: I1490"@en-AU ;
    skos:definition "269 ZZO  Who may seek a review"@en-AU ;
    skos:narrower C1901A00006:1488 ;
    skos:prefLabel "Item I1490"@en-AU ;
    dcat:accessURL "https://www.legislation.gov.au/C1901A00006/2024-07-01/2024-07-01/text/original/epub/OEBPS/document_4/document_4.html#_Toc172628924"^^xsd:anyURI .

C1901A00006:1491 a legcons:Item,
        skos:Concept,
        dcat:Resource ;
    rdfs:label "Item I1491"@en-AU ;
    rdfs:comment "269 ZZP  When must an application be made - GraphNodeID: I1491"@en-AU ;
    skos:definition "269 ZZP  When must an application be made"@en-AU ;
    skos:narrower C1901A00006:1488 ;
    skos:prefLabel "Item I1491"@en-AU ;
    dcat:accessURL "https://www.legislation.gov.au/C1901A00006/2024-07-01/2024-07-01/text/original/epub/OEBPS/document_4/document_4.html#_Toc172628925"^^xsd:anyURI .

C1901A00006:1492 a legcons:Item,
        skos:Concept,
        dcat:Resource ;
    rdfs:label "Item I1492"@en-AU ;
    rdfs:comment "269 ZZQ  How must an application be made - GraphNodeID: I1492"@en-AU ;
    skos:definition "269 ZZQ  How must an application be made"@en-AU ;
    skos:narrower C1901A00006:1488 ;
    skos:prefLabel "Item I1492"@en-AU ;
    dcat:accessURL "https://www.legislation.gov.au/C1901A00006/2024-07-01/2024-07-01/text/original/epub/OEBPS/document_4/document_4.html#_Toc172628926"^^xsd:anyURI .

C1901A00006:1493 a legcons:Item,
        skos:Concept,
        dcat:Resource ;
    rdfs:label "Item I1493"@en-AU ;
    rdfs:comment "269 ZZQAA  Withdrawal of application - GraphNodeID: I1493"@en-AU ;
    skos:definition "269 ZZQAA  Withdrawal of application"@en-AU ;
    skos:narrower C1901A00006:1488 ;
    skos:prefLabel "Item I1493"@en-AU ;
    dcat:accessURL "https://www.legislation.gov.au/C1901A00006/2024-07-01/2024-07-01/text/original/epub/OEBPS/document_4/document_4.html#_Toc172628927"^^xsd:anyURI .

C1901A00006:1494 a legcons:Item,
        skos:Concept,
        dcat:Resource ;
    rdfs:label "Item I1494"@en-AU ;
    rdfs:comment "269 ZZQA  Rejection of applicationfailure to establish decision not the correct or preferable decision etc - GraphNodeID: I1494"@en-AU ;
    skos:definition "269 ZZQA  Rejection of applicationfailure to establish decision not the correct or preferable decision etc"@en-AU ;
    skos:narrower C1901A00006:1488 ;
    skos:prefLabel "Item I1494"@en-AU ;
    dcat:accessURL "https://www.legislation.gov.au/C1901A00006/2024-07-01/2024-07-01/text/original/epub/OEBPS/document_4/document_4.html#_Toc172628928"^^xsd:anyURI .

C1901A00006:1495 a legcons:Item,
        skos:Concept,
        dcat:Resource ;
    rdfs:label "Item I1495"@en-AU ;
    rdfs:comment "269 ZZR  Rejection of application for review of termination decision - GraphNodeID: I1495"@en-AU ;
    skos:definition "269 ZZR  Rejection of application for review of termination decision"@en-AU ;
    skos:narrower C1901A00006:1488 ;
    skos:prefLabel "Item I1495"@en-AU ;
    dcat:accessURL "https://www.legislation.gov.au/C1901A00006/2024-07-01/2024-07-01/text/original/epub/OEBPS/document_4/document_4.html#_Toc172628929"^^xsd:anyURI .

C1901A00006:1496 a legcons:Item,
        skos:Concept,
        dcat:Resource ;
    rdfs:label "Item I1496"@en-AU ;
    rdfs:comment "269 ZZRA  Review Panel may hold conferences - GraphNodeID: I1496"@en-AU ;
    skos:definition "269 ZZRA  Review Panel may hold conferences"@en-AU ;
    skos:narrower C1901A00006:1488 ;
    skos:prefLabel "Item I1496"@en-AU ;
    dcat:accessURL "https://www.legislation.gov.au/C1901A00006/2024-07-01/2024-07-01/text/original/epub/OEBPS/document_4/document_4.html#_Toc172628930"^^xsd:anyURI .

C1901A00006:1497 a legcons:Item,
        skos:Concept,
        dcat:Resource ;
    rdfs:label "Item I1497"@en-AU ;
    rdfs:comment "269 ZZRB  Review Panel may seek further information from the Commissioner - GraphNodeID: I1497"@en-AU ;
    skos:definition "269 ZZRB  Review Panel may seek further information from the Commissioner"@en-AU ;
    skos:narrower C1901A00006:1488 ;
    skos:prefLabel "Item I1497"@en-AU ;
    dcat:accessURL "https://www.legislation.gov.au/C1901A00006/2024-07-01/2024-07-01/text/original/epub/OEBPS/document_4/document_4.html#_Toc172628931"^^xsd:anyURI .

C1901A00006:1498 a legcons:Item,
        skos:Concept,
        dcat:Resource ;
    rdfs:label "Item I1498"@en-AU ;
    rdfs:comment "269 ZZRC  Notification of review - GraphNodeID: I1498"@en-AU ;
    skos:definition "269 ZZRC  Notification of review"@en-AU ;
    skos:narrower C1901A00006:1488 ;
    skos:prefLabel "Item I1498"@en-AU ;
    dcat:accessURL "https://www.legislation.gov.au/C1901A00006/2024-07-01/2024-07-01/text/original/epub/OEBPS/document_4/document_4.html#_Toc172628932"^^xsd:anyURI .

C1901A00006:1499 a legcons:Item,
        skos:Concept,
        dcat:Resource ;
    rdfs:label "Item I1499"@en-AU ;
    rdfs:comment "269 ZZS  The review of a negative prima facie decision - GraphNodeID: I1499"@en-AU ;
    skos:definition "269 ZZS  The review of a negative prima facie decision"@en-AU ;
    skos:narrower C1901A00006:1488 ;
    skos:prefLabel "Item I1499"@en-AU ;
    dcat:accessURL "https://www.legislation.gov.au/C1901A00006/2024-07-01/2024-07-01/text/original/epub/OEBPS/document_4/document_4.html#_Toc172628933"^^xsd:anyURI .

C1901A00006:15 a legcons:Item,
        skos:Concept,
        dcat:Resource ;
    rdfs:label "Item I15"@en-AU ;
    rdfs:comment "5 A  Attachment of overseas resources installations - GraphNodeID: I15"@en-AU ;
    skos:definition "5 A  Attachment of overseas resources installations"@en-AU ;
    skos:narrower C1901A00006:14 ;
    skos:prefLabel "Item I15"@en-AU ;
    dcat:accessURL "https://www.legislation.gov.au/C1901A00006/2024-07-01/2024-07-01/text/original/epub/OEBPS/document_1/document_1.html#_Toc172622989"^^xsd:anyURI .

C1901A00006:150 a legcons:Item,
        skos:Concept,
        dcat:Resource ;
    rdfs:label "Item I150"@en-AU ;
    rdfs:comment "71 A  Making an import declaration - GraphNodeID: I150"@en-AU ;
    skos:definition "71 A  Making an import declaration"@en-AU ;
    skos:narrower C1901A00006:149 ;
    skos:prefLabel "Item I150"@en-AU ;
    dcat:accessURL "https://www.legislation.gov.au/C1901A00006/2024-07-01/2024-07-01/text/original/epub/OEBPS/document_1/document_1.html#_Toc172623124"^^xsd:anyURI .

C1901A00006:1500 a legcons:Item,
        skos:Concept,
        dcat:Resource ;
    rdfs:label "Item I1500"@en-AU ;
    rdfs:comment "269 ZZT  The review of a termination decision - GraphNodeID: I1500"@en-AU ;
    skos:definition "269 ZZT  The review of a termination decision"@en-AU ;
    skos:narrower C1901A00006:1488 ;
    skos:prefLabel "Item I1500"@en-AU ;
    dcat:accessURL "https://www.legislation.gov.au/C1901A00006/2024-07-01/2024-07-01/text/original/epub/OEBPS/document_4/document_4.html#_Toc172628934"^^xsd:anyURI .

C1901A00006:1501 a legcons:Item,
        skos:Concept,
        dcat:Resource ;
    rdfs:label "Item I1501"@en-AU ;
    rdfs:comment "269 ZZU  The review of a negative preliminary decision - GraphNodeID: I1501"@en-AU ;
    skos:definition "269 ZZU  The review of a negative preliminary decision"@en-AU ;
    skos:narrower C1901A00006:1488 ;
    skos:prefLabel "Item I1501"@en-AU ;
    dcat:accessURL "https://www.legislation.gov.au/C1901A00006/2024-07-01/2024-07-01/text/original/epub/OEBPS/document_4/document_4.html#_Toc172628935"^^xsd:anyURI .

C1901A00006:1502 a legcons:Item,
        skos:Concept,
        dcat:Resource ;
    rdfs:label "Item I1502"@en-AU ;
    rdfs:comment "269 ZZUA  The review of a rejection decision - GraphNodeID: I1502"@en-AU ;
    skos:definition "269 ZZUA  The review of a rejection decision"@en-AU ;
    skos:narrower C1901A00006:1488 ;
    skos:prefLabel "Item I1502"@en-AU ;
    dcat:accessURL "https://www.legislation.gov.au/C1901A00006/2024-07-01/2024-07-01/text/original/epub/OEBPS/document_4/document_4.html#_Toc172628936"^^xsd:anyURI .

C1901A00006:1503 a legcons:Item,
        skos:Concept,
        dcat:Resource ;
    rdfs:label "Item I1503"@en-AU ;
    rdfs:comment "269 ZZV  Effect of Review Panels decision - GraphNodeID: I1503"@en-AU ;
    skos:definition "269 ZZV  Effect of Review Panels decision"@en-AU ;
    skos:narrower C1901A00006:1488 ;
    skos:prefLabel "Item I1503"@en-AU ;
    dcat:accessURL "https://www.legislation.gov.au/C1901A00006/2024-07-01/2024-07-01/text/original/epub/OEBPS/document_4/document_4.html#_Toc172628937"^^xsd:anyURI .

C1901A00006:1505 a legcons:Item,
        skos:Concept,
        dcat:Resource ;
    rdfs:label "Item I1505"@en-AU ;
    rdfs:comment "269 ZZW  Application - GraphNodeID: I1505"@en-AU ;
    skos:definition "269 ZZW  Application"@en-AU ;
    skos:narrower C1901A00006:1504 ;
    skos:prefLabel "Item I1505"@en-AU ;
    dcat:accessURL "https://www.legislation.gov.au/C1901A00006/2024-07-01/2024-07-01/text/original/epub/OEBPS/document_4/document_4.html#_Toc172628939"^^xsd:anyURI .

C1901A00006:1506 a legcons:Item,
        skos:Concept,
        dcat:Resource ;
    rdfs:label "Item I1506"@en-AU ;
    rdfs:comment "269 ZZX  Public record maintained by Review Panel - GraphNodeID: I1506"@en-AU ;
    skos:definition "269 ZZX  Public record maintained by Review Panel"@en-AU ;
    skos:narrower C1901A00006:1504 ;
    skos:prefLabel "Item I1506"@en-AU ;
    dcat:accessURL "https://www.legislation.gov.au/C1901A00006/2024-07-01/2024-07-01/text/original/epub/OEBPS/document_4/document_4.html#_Toc172628940"^^xsd:anyURI .

C1901A00006:1507 a legcons:Item,
        skos:Concept,
        dcat:Resource ;
    rdfs:label "Item I1507"@en-AU ;
    rdfs:comment "269 ZZY  Confidential and sensitive commercial information - GraphNodeID: I1507"@en-AU ;
    skos:definition "269 ZZY  Confidential and sensitive commercial information"@en-AU ;
    skos:narrower C1901A00006:1504 ;
    skos:prefLabel "Item I1507"@en-AU ;
    dcat:accessURL "https://www.legislation.gov.au/C1901A00006/2024-07-01/2024-07-01/text/original/epub/OEBPS/document_4/document_4.html#_Toc172628941"^^xsd:anyURI .

C1901A00006:1508 a legcons:Part,
        skos:Concept,
        dcat:Resource ;
    rdfs:label "Part P1508"@en-AU ;
    rdfs:comment "Part XVCInternational Trade Remedies Forum - GraphNodeID: P1508"@en-AU ;
    skos:definition "Part XVCInternational Trade Remedies Forum"@en-AU ;
    skos:narrower C1901A00006:1326 ;
    skos:prefLabel "Part P1508"@en-AU ;
    dcat:accessURL "https://www.legislation.gov.au/C1901A00006/2024-07-01/2024-07-01/text/original/epub/OEBPS/document_4/document_4.html#_Toc172628942"^^xsd:anyURI .

C1901A00006:1509 a legcons:Item,
        skos:Concept,
        dcat:Resource ;
    rdfs:label "Item I1509"@en-AU ;
    rdfs:comment "269 ZZYA  Simplified outline - GraphNodeID: I1509"@en-AU ;
    skos:definition "269 ZZYA  Simplified outline"@en-AU ;
    skos:narrower C1901A00006:1504 ;
    skos:prefLabel "Item I1509"@en-AU ;
    dcat:accessURL "https://www.legislation.gov.au/C1901A00006/2024-07-01/2024-07-01/text/original/epub/OEBPS/document_4/document_4.html#_Toc172628943"^^xsd:anyURI .

C1901A00006:151 a legcons:Item,
        skos:Concept,
        dcat:Resource ;
    rdfs:label "Item I151"@en-AU ;
    rdfs:comment "71 B  Liability for import declaration processing charge - GraphNodeID: I151"@en-AU ;
    skos:definition "71 B  Liability for import declaration processing charge"@en-AU ;
    skos:narrower C1901A00006:149 ;
    skos:prefLabel "Item I151"@en-AU ;
    dcat:accessURL "https://www.legislation.gov.au/C1901A00006/2024-07-01/2024-07-01/text/original/epub/OEBPS/document_1/document_1.html#_Toc172623125"^^xsd:anyURI .

C1901A00006:1510 a legcons:Item,
        skos:Concept,
        dcat:Resource ;
    rdfs:label "Item I1510"@en-AU ;
    rdfs:comment "269 ZZYB  Establishment of International Trade Remedies Forum - GraphNodeID: I1510"@en-AU ;
    skos:definition "269 ZZYB  Establishment of International Trade Remedies Forum"@en-AU ;
    skos:narrower C1901A00006:1504 ;
    skos:prefLabel "Item I1510"@en-AU ;
    dcat:accessURL "https://www.legislation.gov.au/C1901A00006/2024-07-01/2024-07-01/text/original/epub/OEBPS/document_4/document_4.html#_Toc172628944"^^xsd:anyURI .

C1901A00006:1511 a legcons:Item,
        skos:Concept,
        dcat:Resource ;
    rdfs:label "Item I1511"@en-AU ;
    rdfs:comment "269 ZZYC  Functions of the Forum - GraphNodeID: I1511"@en-AU ;
    skos:definition "269 ZZYC  Functions of the Forum"@en-AU ;
    skos:narrower C1901A00006:1504 ;
    skos:prefLabel "Item I1511"@en-AU ;
    dcat:accessURL "https://www.legislation.gov.au/C1901A00006/2024-07-01/2024-07-01/text/original/epub/OEBPS/document_4/document_4.html#_Toc172628945"^^xsd:anyURI .

C1901A00006:1512 a legcons:Item,
        skos:Concept,
        dcat:Resource ;
    rdfs:label "Item I1512"@en-AU ;
    rdfs:comment "269 ZZYD  Membership of the Forum - GraphNodeID: I1512"@en-AU ;
    skos:definition "269 ZZYD  Membership of the Forum"@en-AU ;
    skos:narrower C1901A00006:1504 ;
    skos:prefLabel "Item I1512"@en-AU ;
    dcat:accessURL "https://www.legislation.gov.au/C1901A00006/2024-07-01/2024-07-01/text/original/epub/OEBPS/document_4/document_4.html#_Toc172628946"^^xsd:anyURI .

C1901A00006:1513 a legcons:Item,
        skos:Concept,
        dcat:Resource ;
    rdfs:label "Item I1513"@en-AU ;
    rdfs:comment "269 ZZYE  Appointment of Forum members - GraphNodeID: I1513"@en-AU ;
    skos:definition "269 ZZYE  Appointment of Forum members"@en-AU ;
    skos:narrower C1901A00006:1504 ;
    skos:prefLabel "Item I1513"@en-AU ;
    dcat:accessURL "https://www.legislation.gov.au/C1901A00006/2024-07-01/2024-07-01/text/original/epub/OEBPS/document_4/document_4.html#_Toc172628947"^^xsd:anyURI .

C1901A00006:1514 a legcons:Item,
        skos:Concept,
        dcat:Resource ;
    rdfs:label "Item I1514"@en-AU ;
    rdfs:comment "269 ZZYF  Resignation - GraphNodeID: I1514"@en-AU ;
    skos:definition "269 ZZYF  Resignation"@en-AU ;
    skos:narrower C1901A00006:1504 ;
    skos:prefLabel "Item I1514"@en-AU ;
    dcat:accessURL "https://www.legislation.gov.au/C1901A00006/2024-07-01/2024-07-01/text/original/epub/OEBPS/document_4/document_4.html#_Toc172628948"^^xsd:anyURI .

C1901A00006:1515 a legcons:Item,
        skos:Concept,
        dcat:Resource ;
    rdfs:label "Item I1515"@en-AU ;
    rdfs:comment "269 ZZYG  Forum meetings - GraphNodeID: I1515"@en-AU ;
    skos:definition "269 ZZYG  Forum meetings"@en-AU ;
    skos:narrower C1901A00006:1504 ;
    skos:prefLabel "Item I1515"@en-AU ;
    dcat:accessURL "https://www.legislation.gov.au/C1901A00006/2024-07-01/2024-07-01/text/original/epub/OEBPS/document_4/document_4.html#_Toc172628949"^^xsd:anyURI .

C1901A00006:1516 a legcons:Item,
        skos:Concept,
        dcat:Resource ;
    rdfs:label "Item I1516"@en-AU ;
    rdfs:comment "269 ZZYH  Disclosure of information - GraphNodeID: I1516"@en-AU ;
    skos:definition "269 ZZYH  Disclosure of information"@en-AU ;
    skos:narrower C1901A00006:1504 ;
    skos:prefLabel "Item I1516"@en-AU ;
    dcat:accessURL "https://www.legislation.gov.au/C1901A00006/2024-07-01/2024-07-01/text/original/epub/OEBPS/document_4/document_4.html#_Toc172628950"^^xsd:anyURI .

C1901A00006:1517 a legcons:Part,
        skos:Concept,
        dcat:Resource ;
    rdfs:label "Part P1517"@en-AU ;
    rdfs:comment "Part XVIRegulations and by laws - GraphNodeID: P1517"@en-AU ;
    skos:definition "Part XVIRegulations and by laws"@en-AU ;
    skos:narrower C1901A00006:1326 ;
    skos:prefLabel "Part P1517"@en-AU ;
    dcat:accessURL "https://www.legislation.gov.au/C1901A00006/2024-07-01/2024-07-01/text/original/epub/OEBPS/document_4/document_4.html#_Toc172628951"^^xsd:anyURI .

C1901A00006:1518 a legcons:Item,
        skos:Concept,
        dcat:Resource ;
    rdfs:label "Item I1518"@en-AU ;
    rdfs:comment "270  Regulations - GraphNodeID: I1518"@en-AU ;
    skos:definition "270  Regulations"@en-AU ;
    skos:narrower C1901A00006:1504 ;
    skos:prefLabel "Item I1518"@en-AU ;
    dcat:accessURL "https://www.legislation.gov.au/C1901A00006/2024-07-01/2024-07-01/text/original/epub/OEBPS/document_4/document_4.html#_Toc172628952"^^xsd:anyURI .

C1901A00006:1519 a legcons:Item,
        skos:Concept,
        dcat:Resource ;
    rdfs:label "Item I1519"@en-AU ;
    rdfs:comment "271  Comptroller General of Customs may make by laws - GraphNodeID: I1519"@en-AU ;
    skos:definition "271  Comptroller General of Customs may make by laws"@en-AU ;
    skos:narrower C1901A00006:1504 ;
    skos:prefLabel "Item I1519"@en-AU ;
    dcat:accessURL "https://www.legislation.gov.au/C1901A00006/2024-07-01/2024-07-01/text/original/epub/OEBPS/document_4/document_4.html#_Toc172628953"^^xsd:anyURI .

C1901A00006:152 a legcons:Item,
        skos:Concept,
        dcat:Resource ;
    rdfs:label "Item I152"@en-AU ;
    rdfs:comment "71 BA  Warehoused goods declaration fee - GraphNodeID: I152"@en-AU ;
    skos:definition "71 BA  Warehoused goods declaration fee"@en-AU ;
    skos:narrower C1901A00006:149 ;
    skos:prefLabel "Item I152"@en-AU ;
    dcat:accessURL "https://www.legislation.gov.au/C1901A00006/2024-07-01/2024-07-01/text/original/epub/OEBPS/document_1/document_1.html#_Toc172623126"^^xsd:anyURI .

C1901A00006:1520 a legcons:Item,
        skos:Concept,
        dcat:Resource ;
    rdfs:label "Item I1520"@en-AU ;
    rdfs:comment "272  By laws specifying goods - GraphNodeID: I1520"@en-AU ;
    skos:definition "272  By laws specifying goods"@en-AU ;
    skos:narrower C1901A00006:1504 ;
    skos:prefLabel "Item I1520"@en-AU ;
    dcat:accessURL "https://www.legislation.gov.au/C1901A00006/2024-07-01/2024-07-01/text/original/epub/OEBPS/document_4/document_4.html#_Toc172628954"^^xsd:anyURI .

C1901A00006:1521 a legcons:Item,
        skos:Concept,
        dcat:Resource ;
    rdfs:label "Item I1521"@en-AU ;
    rdfs:comment "273  Determinations - GraphNodeID: I1521"@en-AU ;
    skos:definition "273  Determinations"@en-AU ;
    skos:narrower C1901A00006:1504 ;
    skos:prefLabel "Item I1521"@en-AU ;
    dcat:accessURL "https://www.legislation.gov.au/C1901A00006/2024-07-01/2024-07-01/text/original/epub/OEBPS/document_4/document_4.html#_Toc172628955"^^xsd:anyURI .

C1901A00006:1522 a legcons:Item,
        skos:Concept,
        dcat:Resource ;
    rdfs:label "Item I1522"@en-AU ;
    rdfs:comment "273 A  By laws and determinations for purposes of repealed items - GraphNodeID: I1522"@en-AU ;
    skos:definition "273 A  By laws and determinations for purposes of repealed items"@en-AU ;
    skos:narrower C1901A00006:1504 ;
    skos:prefLabel "Item I1522"@en-AU ;
    dcat:accessURL "https://www.legislation.gov.au/C1901A00006/2024-07-01/2024-07-01/text/original/epub/OEBPS/document_4/document_4.html#_Toc172628956"^^xsd:anyURI .

C1901A00006:1523 a legcons:Item,
        skos:Concept,
        dcat:Resource ;
    rdfs:label "Item I1523"@en-AU ;
    rdfs:comment "273 B  Publication of by laws and notification of determinations - GraphNodeID: I1523"@en-AU ;
    skos:definition "273 B  Publication of by laws and notification of determinations"@en-AU ;
    skos:narrower C1901A00006:1504 ;
    skos:prefLabel "Item I1523"@en-AU ;
    dcat:accessURL "https://www.legislation.gov.au/C1901A00006/2024-07-01/2024-07-01/text/original/epub/OEBPS/document_4/document_4.html#_Toc172628957"^^xsd:anyURI .

C1901A00006:1524 a legcons:Item,
        skos:Concept,
        dcat:Resource ;
    rdfs:label "Item I1524"@en-AU ;
    rdfs:comment "273 C  Retrospective by laws and determinations not to increase duty - GraphNodeID: I1524"@en-AU ;
    skos:definition "273 C  Retrospective by laws and determinations not to increase duty"@en-AU ;
    skos:narrower C1901A00006:1504 ;
    skos:prefLabel "Item I1524"@en-AU ;
    dcat:accessURL "https://www.legislation.gov.au/C1901A00006/2024-07-01/2024-07-01/text/original/epub/OEBPS/document_4/document_4.html#_Toc172628958"^^xsd:anyURI .

C1901A00006:1525 a legcons:Item,
        skos:Concept,
        dcat:Resource ;
    rdfs:label "Item I1525"@en-AU ;
    rdfs:comment "273 D  By laws and determinations for purposes of proposals - GraphNodeID: I1525"@en-AU ;
    skos:definition "273 D  By laws and determinations for purposes of proposals"@en-AU ;
    skos:narrower C1901A00006:1504 ;
    skos:prefLabel "Item I1525"@en-AU ;
    dcat:accessURL "https://www.legislation.gov.au/C1901A00006/2024-07-01/2024-07-01/text/original/epub/OEBPS/document_4/document_4.html#_Toc172628959"^^xsd:anyURI .

C1901A00006:1526 a legcons:Item,
        skos:Concept,
        dcat:Resource ;
    rdfs:label "Item I1526"@en-AU ;
    rdfs:comment "273 EA  Notification of proposals when House of Representatives is not sitting - GraphNodeID: I1526"@en-AU ;
    skos:definition "273 EA  Notification of proposals when House of Representatives is not sitting"@en-AU ;
    skos:narrower C1901A00006:1504 ;
    skos:prefLabel "Item I1526"@en-AU ;
    dcat:accessURL "https://www.legislation.gov.au/C1901A00006/2024-07-01/2024-07-01/text/original/epub/OEBPS/document_4/document_4.html#_Toc172628960"^^xsd:anyURI .

C1901A00006:1527 a legcons:Item,
        skos:Concept,
        dcat:Resource ;
    rdfs:label "Item I1527"@en-AU ;
    rdfs:comment "273 F  Interpretation - GraphNodeID: I1527"@en-AU ;
    skos:definition "273 F  Interpretation"@en-AU ;
    skos:narrower C1901A00006:1504 ;
    skos:prefLabel "Item I1527"@en-AU ;
    dcat:accessURL "https://www.legislation.gov.au/C1901A00006/2024-07-01/2024-07-01/text/original/epub/OEBPS/document_4/document_4.html#_Toc172628961"^^xsd:anyURI .

C1901A00006:1528 a legcons:Part,
        skos:Concept,
        dcat:Resource ;
    rdfs:label "Part P1528"@en-AU ;
    rdfs:comment "Part XVIIMiscellaneous - GraphNodeID: P1528"@en-AU ;
    skos:definition "Part XVIIMiscellaneous"@en-AU ;
    skos:narrower C1901A00006:1326 ;
    skos:prefLabel "Part P1528"@en-AU ;
    dcat:accessURL "https://www.legislation.gov.au/C1901A00006/2024-07-01/2024-07-01/text/original/epub/OEBPS/document_4/document_4.html#_Toc172628962"^^xsd:anyURI .

C1901A00006:1529 a legcons:Item,
        skos:Concept,
        dcat:Resource ;
    rdfs:label "Item I1529"@en-AU ;
    rdfs:comment "273 G  Briefing of Leader of Opposition on certain matters - GraphNodeID: I1529"@en-AU ;
    skos:definition "273 G  Briefing of Leader of Opposition on certain matters"@en-AU ;
    skos:narrower C1901A00006:1504 ;
    skos:prefLabel "Item I1529"@en-AU ;
    dcat:accessURL "https://www.legislation.gov.au/C1901A00006/2024-07-01/2024-07-01/text/original/epub/OEBPS/document_4/document_4.html#_Toc172628963"^^xsd:anyURI .

C1901A00006:153 a legcons:Item,
        skos:Concept,
        dcat:Resource ;
    rdfs:label "Item I153"@en-AU ;
    rdfs:comment "71 C  Authority to deal with goods in respect of which an import declaration has been made - GraphNodeID: I153"@en-AU ;
    skos:definition "71 C  Authority to deal with goods in respect of which an import declaration has been made"@en-AU ;
    skos:narrower C1901A00006:149 ;
    skos:prefLabel "Item I153"@en-AU ;
    dcat:accessURL "https://www.legislation.gov.au/C1901A00006/2024-07-01/2024-07-01/text/original/epub/OEBPS/document_1/document_1.html#_Toc172623127"^^xsd:anyURI .

C1901A00006:1530 a legcons:Item,
        skos:Concept,
        dcat:Resource ;
    rdfs:label "Item I1530"@en-AU ;
    rdfs:comment "273 GAA  Notices - GraphNodeID: I1530"@en-AU ;
    skos:definition "273 GAA  Notices"@en-AU ;
    skos:narrower C1901A00006:1504 ;
    skos:prefLabel "Item I1530"@en-AU ;
    dcat:accessURL "https://www.legislation.gov.au/C1901A00006/2024-07-01/2024-07-01/text/original/epub/OEBPS/document_4/document_4.html#_Toc172628964"^^xsd:anyURI .

C1901A00006:1531 a legcons:Item,
        skos:Concept,
        dcat:Resource ;
    rdfs:label "Item I1531"@en-AU ;
    rdfs:comment "273 GAB  Authorisation to disclose information to an officer - GraphNodeID: I1531"@en-AU ;
    skos:definition "273 GAB  Authorisation to disclose information to an officer"@en-AU ;
    skos:narrower C1901A00006:1504 ;
    skos:prefLabel "Item I1531"@en-AU ;
    dcat:accessURL "https://www.legislation.gov.au/C1901A00006/2024-07-01/2024-07-01/text/original/epub/OEBPS/document_4/document_4.html#_Toc172628965"^^xsd:anyURI .

C1901A00006:1532 a legcons:Item,
        skos:Concept,
        dcat:Resource ;
    rdfs:label "Item I1532"@en-AU ;
    rdfs:comment "273 GA  Review of decisions - GraphNodeID: I1532"@en-AU ;
    skos:definition "273 GA  Review of decisions"@en-AU ;
    skos:narrower C1901A00006:1504 ;
    skos:prefLabel "Item I1532"@en-AU ;
    dcat:accessURL "https://www.legislation.gov.au/C1901A00006/2024-07-01/2024-07-01/text/original/epub/OEBPS/document_4/document_4.html#_Toc172628966"^^xsd:anyURI .

C1901A00006:1533 a legcons:Item,
        skos:Concept,
        dcat:Resource ;
    rdfs:label "Item I1533"@en-AU ;
    rdfs:comment "273 H  Review of decisions under Customs Tariff Act - GraphNodeID: I1533"@en-AU ;
    skos:definition "273 H  Review of decisions under Customs Tariff Act"@en-AU ;
    skos:narrower C1901A00006:1504 ;
    skos:prefLabel "Item I1533"@en-AU ;
    dcat:accessURL "https://www.legislation.gov.au/C1901A00006/2024-07-01/2024-07-01/text/original/epub/OEBPS/document_4/document_4.html#_Toc172628967"^^xsd:anyURI .

C1901A00006:1534 a legcons:Item,
        skos:Concept,
        dcat:Resource ;
    rdfs:label "Item I1534"@en-AU ;
    rdfs:comment "273 K  Statement to accompany notification of decisions - GraphNodeID: I1534"@en-AU ;
    skos:definition "273 K  Statement to accompany notification of decisions"@en-AU ;
    skos:narrower C1901A00006:1504 ;
    skos:prefLabel "Item I1534"@en-AU ;
    dcat:accessURL "https://www.legislation.gov.au/C1901A00006/2024-07-01/2024-07-01/text/original/epub/OEBPS/document_4/document_4.html#_Toc172628968"^^xsd:anyURI .

C1901A00006:1535 a legcons:Item,
        skos:Concept,
        dcat:Resource ;
    rdfs:label "Item I1535"@en-AU ;
    rdfs:comment "273 L  Entry and transmission of information by computer - GraphNodeID: I1535"@en-AU ;
    skos:definition "273 L  Entry and transmission of information by computer"@en-AU ;
    skos:narrower C1901A00006:1504 ;
    skos:prefLabel "Item I1535"@en-AU ;
    dcat:accessURL "https://www.legislation.gov.au/C1901A00006/2024-07-01/2024-07-01/text/original/epub/OEBPS/document_4/document_4.html#_Toc172628969"^^xsd:anyURI .

C1901A00006:1536 a legcons:Item,
        skos:Concept,
        dcat:Resource ;
    rdfs:label "Item I1536"@en-AU ;
    rdfs:comment "274  Commissioned ships and aircraft to be reported - GraphNodeID: I1536"@en-AU ;
    skos:definition "274  Commissioned ships and aircraft to be reported"@en-AU ;
    skos:narrower C1901A00006:1504 ;
    skos:prefLabel "Item I1536"@en-AU ;
    dcat:accessURL "https://www.legislation.gov.au/C1901A00006/2024-07-01/2024-07-01/text/original/epub/OEBPS/document_4/document_4.html#_Toc172628970"^^xsd:anyURI .

C1901A00006:1537 a legcons:Item,
        skos:Concept,
        dcat:Resource ;
    rdfs:label "Item I1537"@en-AU ;
    rdfs:comment "275  Commissioned ships and aircraft may be searched - GraphNodeID: I1537"@en-AU ;
    skos:definition "275  Commissioned ships and aircraft may be searched"@en-AU ;
    skos:narrower C1901A00006:1504 ;
    skos:prefLabel "Item I1537"@en-AU ;
    dcat:accessURL "https://www.legislation.gov.au/C1901A00006/2024-07-01/2024-07-01/text/original/epub/OEBPS/document_4/document_4.html#_Toc172628971"^^xsd:anyURI .

C1901A00006:1538 a legcons:Item,
        skos:Concept,
        dcat:Resource ;
    rdfs:label "Item I1538"@en-AU ;
    rdfs:comment "275 A  Direction not to move a ship or aircraft from a boarding station - GraphNodeID: I1538"@en-AU ;
    skos:definition "275 A  Direction not to move a ship or aircraft from a boarding station"@en-AU ;
    skos:narrower C1901A00006:1504 ;
    skos:prefLabel "Item I1538"@en-AU ;
    dcat:accessURL "https://www.legislation.gov.au/C1901A00006/2024-07-01/2024-07-01/text/original/epub/OEBPS/document_4/document_4.html#_Toc172628972"^^xsd:anyURI .

C1901A00006:1539 a legcons:Item,
        skos:Concept,
        dcat:Resource ;
    rdfs:label "Item I1539"@en-AU ;
    rdfs:comment "276  Collectors sales - GraphNodeID: I1539"@en-AU ;
    skos:definition "276  Collectors sales"@en-AU ;
    skos:narrower C1901A00006:1504 ;
    skos:prefLabel "Item I1539"@en-AU ;
    dcat:accessURL "https://www.legislation.gov.au/C1901A00006/2024-07-01/2024-07-01/text/original/epub/OEBPS/document_4/document_4.html#_Toc172628973"^^xsd:anyURI .

C1901A00006:154 a legcons:Item,
        skos:Concept,
        dcat:Resource ;
    rdfs:label "Item I154"@en-AU ;
    rdfs:comment "71 D  Visual examination in presence of officer - GraphNodeID: I154"@en-AU ;
    skos:definition "71 D  Visual examination in presence of officer"@en-AU ;
    skos:narrower C1901A00006:149 ;
    skos:prefLabel "Item I154"@en-AU ;
    dcat:accessURL "https://www.legislation.gov.au/C1901A00006/2024-07-01/2024-07-01/text/original/epub/OEBPS/document_1/document_1.html#_Toc172623128"^^xsd:anyURI .

C1901A00006:1540 a legcons:Item,
        skos:Concept,
        dcat:Resource ;
    rdfs:label "Item I1540"@en-AU ;
    rdfs:comment "277  Proceeds of sales - GraphNodeID: I1540"@en-AU ;
    skos:definition "277  Proceeds of sales"@en-AU ;
    skos:narrower C1901A00006:1504 ;
    skos:prefLabel "Item I1540"@en-AU ;
    dcat:accessURL "https://www.legislation.gov.au/C1901A00006/2024-07-01/2024-07-01/text/original/epub/OEBPS/document_4/document_4.html#_Toc172628974"^^xsd:anyURI .

C1901A00006:1541 a legcons:Item,
        skos:Concept,
        dcat:Resource ;
    rdfs:label "Item I1541"@en-AU ;
    rdfs:comment "277 A  Jurisdiction of courts - GraphNodeID: I1541"@en-AU ;
    skos:definition "277 A  Jurisdiction of courts"@en-AU ;
    skos:narrower C1901A00006:1504 ;
    skos:prefLabel "Item I1541"@en-AU ;
    dcat:accessURL "https://www.legislation.gov.au/C1901A00006/2024-07-01/2024-07-01/text/original/epub/OEBPS/document_4/document_4.html#_Toc172628975"^^xsd:anyURI .

C1901A00006:1542 a legcons:Item,
        skos:Concept,
        dcat:Resource ;
    rdfs:label "Item I1542"@en-AU ;
    rdfs:comment "278  Recoverable payments - GraphNodeID: I1542"@en-AU ;
    skos:definition "278  Recoverable payments"@en-AU ;
    skos:narrower C1901A00006:1504 ;
    skos:prefLabel "Item I1542"@en-AU ;
    dcat:accessURL "https://www.legislation.gov.au/C1901A00006/2024-07-01/2024-07-01/text/original/epub/OEBPS/document_4/document_4.html#_Toc172628976"^^xsd:anyURI .

C1901A00006:1543 a legcons:Item,
        skos:Concept,
        dcat:Resource ;
    rdfs:label "Item I1543"@en-AU ;
    rdfs:comment "279  Reports about recoverable payments - GraphNodeID: I1543"@en-AU ;
    skos:definition "279  Reports about recoverable payments"@en-AU ;
    skos:narrower C1901A00006:1504 ;
    skos:prefLabel "Item I1543"@en-AU ;
    dcat:accessURL "https://www.legislation.gov.au/C1901A00006/2024-07-01/2024-07-01/text/original/epub/OEBPS/document_4/document_4.html#_Toc172628977"^^xsd:anyURI .

C1901A00006:1544 a legcons:Item,
        skos:Concept,
        dcat:Resource ;
    rdfs:label "Item I1544"@en-AU ;
    rdfs:comment "Schedule IThe Commonwealth of Australia - GraphNodeID: I1544"@en-AU ;
    skos:definition "Schedule IThe Commonwealth of Australia"@en-AU ;
    skos:narrower C1901A00006:1504 ;
    skos:prefLabel "Item I1544"@en-AU ;
    dcat:accessURL "https://www.legislation.gov.au/C1901A00006/2024-07-01/2024-07-01/text/original/epub/OEBPS/document_4/document_4.html#_Toc172628978"^^xsd:anyURI .

C1901A00006:1545 a legcons:Volume,
        skos:Concept,
        dcat:Resource ;
    rdfs:label "Volume V1545"@en-AU ;
    rdfs:comment "Volume 5 - GraphNodeID: V1545"@en-AU ;
    skos:broader C1901A00006:1546 ;
    skos:definition "Volume 5"@en-AU ;
    skos:prefLabel "Volume V1545"@en-AU ;
    dcat:accessURL "https://www.legislation.gov.au/C1901A00006/2024-07-01/2024-07-01/text/original/epub/OEBPS/document_5/document_5.html"^^xsd:anyURI .

C1901A00006:1546 a legcons:Part,
        skos:Concept,
        dcat:Resource ;
    rdfs:label "Part P1546"@en-AU ;
    rdfs:comment "Endnotes - GraphNodeID: P1546"@en-AU ;
    skos:definition "Endnotes"@en-AU ;
    skos:narrower C1901A00006:1545 ;
    skos:prefLabel "Part P1546"@en-AU ;
    dcat:accessURL "https://www.legislation.gov.au/C1901A00006/2024-07-01/2024-07-01/text/original/epub/OEBPS/document_5/document_5.html#_Toc172616126"^^xsd:anyURI .

C1901A00006:1547 a legcons:Item,
        skos:Concept,
        dcat:Resource ;
    rdfs:label "Item I1547"@en-AU ;
    rdfs:comment "Endnote 1 About the endnotes - GraphNodeID: I1547"@en-AU ;
    skos:definition "Endnote 1 About the endnotes"@en-AU ;
    skos:narrower C1901A00006:1504 ;
    skos:prefLabel "Item I1547"@en-AU ;
    dcat:accessURL "https://www.legislation.gov.au/C1901A00006/2024-07-01/2024-07-01/text/original/epub/OEBPS/document_5/document_5.html#_Toc172616127"^^xsd:anyURI .

C1901A00006:1548 a legcons:Item,
        skos:Concept,
        dcat:Resource ;
    rdfs:label "Item I1548"@en-AU ;
    rdfs:comment "Endnote 2 Abbreviation key - GraphNodeID: I1548"@en-AU ;
    skos:definition "Endnote 2 Abbreviation key"@en-AU ;
    skos:narrower C1901A00006:1504 ;
    skos:prefLabel "Item I1548"@en-AU ;
    dcat:accessURL "https://www.legislation.gov.au/C1901A00006/2024-07-01/2024-07-01/text/original/epub/OEBPS/document_5/document_5.html#_Toc172616128"^^xsd:anyURI .

C1901A00006:1549 a legcons:Item,
        skos:Concept,
        dcat:Resource ;
    rdfs:label "Item I1549"@en-AU ;
    rdfs:comment "Endnote 3 Legislation history - GraphNodeID: I1549"@en-AU ;
    skos:definition "Endnote 3 Legislation history"@en-AU ;
    skos:narrower C1901A00006:1504 ;
    skos:prefLabel "Item I1549"@en-AU ;
    dcat:accessURL "https://www.legislation.gov.au/C1901A00006/2024-07-01/2024-07-01/text/original/epub/OEBPS/document_5/document_5.html#_Toc172616129"^^xsd:anyURI .

C1901A00006:155 a legcons:Item,
        skos:Concept,
        dcat:Resource ;
    rdfs:label "Item I155"@en-AU ;
    rdfs:comment "71 DA  An officer may seek additional information - GraphNodeID: I155"@en-AU ;
    skos:definition "71 DA  An officer may seek additional information"@en-AU ;
    skos:narrower C1901A00006:149 ;
    skos:prefLabel "Item I155"@en-AU ;
    dcat:accessURL "https://www.legislation.gov.au/C1901A00006/2024-07-01/2024-07-01/text/original/epub/OEBPS/document_1/document_1.html#_Toc172623129"^^xsd:anyURI .

C1901A00006:1550 a legcons:Item,
        skos:Concept,
        dcat:Resource ;
    rdfs:label "Item I1550"@en-AU ;
    rdfs:comment "Endnote 4 Amendment history - GraphNodeID: I1550"@en-AU ;
    skos:definition "Endnote 4 Amendment history"@en-AU ;
    skos:narrower C1901A00006:1504 ;
    skos:prefLabel "Item I1550"@en-AU ;
    dcat:accessURL "https://www.legislation.gov.au/C1901A00006/2024-07-01/2024-07-01/text/original/epub/OEBPS/document_5/document_5.html#_Toc172616130"^^xsd:anyURI .

C1901A00006:1551 a legcons:Item,
        skos:Concept,
        dcat:Resource ;
    rdfs:label "Item I1551"@en-AU ;
    rdfs:comment "Endnote 5 Editorial changes - GraphNodeID: I1551"@en-AU ;
    skos:definition "Endnote 5 Editorial changes"@en-AU ;
    skos:narrower C1901A00006:1504 ;
    skos:prefLabel "Item I1551"@en-AU ;
    dcat:accessURL "https://www.legislation.gov.au/C1901A00006/2024-07-01/2024-07-01/text/original/epub/OEBPS/document_5/document_5.html#_Toc172616131"^^xsd:anyURI .

C1901A00006:157 a legcons:Item,
        skos:Concept,
        dcat:Resource ;
    rdfs:label "Item I157"@en-AU ;
    rdfs:comment "71 DG  Subdivision does not apply to tobacco products - GraphNodeID: I157"@en-AU ;
    skos:definition "71 DG  Subdivision does not apply to tobacco products"@en-AU ;
    skos:narrower C1901A00006:156 ;
    skos:prefLabel "Item I157"@en-AU ;
    dcat:accessURL "https://www.legislation.gov.au/C1901A00006/2024-07-01/2024-07-01/text/original/epub/OEBPS/document_1/document_1.html#_Toc172623131"^^xsd:anyURI .

C1901A00006:158 a legcons:Item,
        skos:Concept,
        dcat:Resource ;
    rdfs:label "Item I158"@en-AU ;
    rdfs:comment "71 DH  Making a warehouse declaration - GraphNodeID: I158"@en-AU ;
    skos:definition "71 DH  Making a warehouse declaration"@en-AU ;
    skos:narrower C1901A00006:156 ;
    skos:prefLabel "Item I158"@en-AU ;
    dcat:accessURL "https://www.legislation.gov.au/C1901A00006/2024-07-01/2024-07-01/text/original/epub/OEBPS/document_1/document_1.html#_Toc172623132"^^xsd:anyURI .

C1901A00006:159 a legcons:Item,
        skos:Concept,
        dcat:Resource ;
    rdfs:label "Item I159"@en-AU ;
    rdfs:comment "71 DI  Liability for warehouse declaration processing charge - GraphNodeID: I159"@en-AU ;
    skos:definition "71 DI  Liability for warehouse declaration processing charge"@en-AU ;
    skos:narrower C1901A00006:156 ;
    skos:prefLabel "Item I159"@en-AU ;
    dcat:accessURL "https://www.legislation.gov.au/C1901A00006/2024-07-01/2024-07-01/text/original/epub/OEBPS/document_1/document_1.html#_Toc172623133"^^xsd:anyURI .

C1901A00006:16 a legcons:Item,
        skos:Concept,
        dcat:Resource ;
    rdfs:label "Item I16"@en-AU ;
    rdfs:comment "5 B  Installation of overseas sea installations - GraphNodeID: I16"@en-AU ;
    skos:definition "5 B  Installation of overseas sea installations"@en-AU ;
    skos:narrower C1901A00006:14 ;
    skos:prefLabel "Item I16"@en-AU ;
    dcat:accessURL "https://www.legislation.gov.au/C1901A00006/2024-07-01/2024-07-01/text/original/epub/OEBPS/document_1/document_1.html#_Toc172622990"^^xsd:anyURI .

C1901A00006:160 a legcons:Item,
        skos:Concept,
        dcat:Resource ;
    rdfs:label "Item I160"@en-AU ;
    rdfs:comment "71 DJ  Authority to deal with goods in respect of which a warehouse declaration has been made - GraphNodeID: I160"@en-AU ;
    skos:definition "71 DJ  Authority to deal with goods in respect of which a warehouse declaration has been made"@en-AU ;
    skos:narrower C1901A00006:156 ;
    skos:prefLabel "Item I160"@en-AU ;
    dcat:accessURL "https://www.legislation.gov.au/C1901A00006/2024-07-01/2024-07-01/text/original/epub/OEBPS/document_1/document_1.html#_Toc172623134"^^xsd:anyURI .

C1901A00006:161 a legcons:Item,
        skos:Concept,
        dcat:Resource ;
    rdfs:label "Item I161"@en-AU ;
    rdfs:comment "71 DK  Visual examination in presence of officer - GraphNodeID: I161"@en-AU ;
    skos:definition "71 DK  Visual examination in presence of officer"@en-AU ;
    skos:narrower C1901A00006:156 ;
    skos:prefLabel "Item I161"@en-AU ;
    dcat:accessURL "https://www.legislation.gov.au/C1901A00006/2024-07-01/2024-07-01/text/original/epub/OEBPS/document_1/document_1.html#_Toc172623135"^^xsd:anyURI .

C1901A00006:162 a legcons:Item,
        skos:Concept,
        dcat:Resource ;
    rdfs:label "Item I162"@en-AU ;
    rdfs:comment "71 DL  An officer may seek additional information - GraphNodeID: I162"@en-AU ;
    skos:definition "71 DL  An officer may seek additional information"@en-AU ;
    skos:narrower C1901A00006:156 ;
    skos:prefLabel "Item I162"@en-AU ;
    dcat:accessURL "https://www.legislation.gov.au/C1901A00006/2024-07-01/2024-07-01/text/original/epub/OEBPS/document_1/document_1.html#_Toc172623136"^^xsd:anyURI .

C1901A00006:164 a legcons:Item,
        skos:Concept,
        dcat:Resource ;
    rdfs:label "Item I164"@en-AU ;
    rdfs:comment "71 E  Movement permissions - GraphNodeID: I164"@en-AU ;
    skos:definition "71 E  Movement permissions"@en-AU ;
    skos:narrower C1901A00006:163 ;
    skos:prefLabel "Item I164"@en-AU ;
    dcat:accessURL "https://www.legislation.gov.au/C1901A00006/2024-07-01/2024-07-01/text/original/epub/OEBPS/document_1/document_1.html#_Toc172623138"^^xsd:anyURI .

C1901A00006:165 a legcons:Item,
        skos:Concept,
        dcat:Resource ;
    rdfs:label "Item I165"@en-AU ;
    rdfs:comment "71 F  Withdrawal of import entries - GraphNodeID: I165"@en-AU ;
    skos:definition "71 F  Withdrawal of import entries"@en-AU ;
    skos:narrower C1901A00006:163 ;
    skos:prefLabel "Item I165"@en-AU ;
    dcat:accessURL "https://www.legislation.gov.au/C1901A00006/2024-07-01/2024-07-01/text/original/epub/OEBPS/document_1/document_1.html#_Toc172623139"^^xsd:anyURI .

C1901A00006:166 a legcons:Item,
        skos:Concept,
        dcat:Resource ;
    rdfs:label "Item I166"@en-AU ;
    rdfs:comment "71 G  Goods not to be entered while an entry is outstanding - GraphNodeID: I166"@en-AU ;
    skos:definition "71 G  Goods not to be entered while an entry is outstanding"@en-AU ;
    skos:narrower C1901A00006:163 ;
    skos:prefLabel "Item I166"@en-AU ;
    dcat:accessURL "https://www.legislation.gov.au/C1901A00006/2024-07-01/2024-07-01/text/original/epub/OEBPS/document_1/document_1.html#_Toc172623140"^^xsd:anyURI .

C1901A00006:167 a legcons:Item,
        skos:Concept,
        dcat:Resource ;
    rdfs:label "Item I167"@en-AU ;
    rdfs:comment "71 H  Effect of withdrawal - GraphNodeID: I167"@en-AU ;
    skos:definition "71 H  Effect of withdrawal"@en-AU ;
    skos:narrower C1901A00006:163 ;
    skos:prefLabel "Item I167"@en-AU ;
    dcat:accessURL "https://www.legislation.gov.au/C1901A00006/2024-07-01/2024-07-01/text/original/epub/OEBPS/document_1/document_1.html#_Toc172623141"^^xsd:anyURI .

C1901A00006:168 a legcons:Item,
        skos:Concept,
        dcat:Resource ;
    rdfs:label "Item I168"@en-AU ;
    rdfs:comment "71 J  Annotation of import entry by Collector for certain purposes not to constitute withdrawal - GraphNodeID: I168"@en-AU ;
    skos:definition "71 J  Annotation of import entry by Collector for certain purposes not to constitute withdrawal"@en-AU ;
    skos:narrower C1901A00006:163 ;
    skos:prefLabel "Item I168"@en-AU ;
    dcat:accessURL "https://www.legislation.gov.au/C1901A00006/2024-07-01/2024-07-01/text/original/epub/OEBPS/document_1/document_1.html#_Toc172623142"^^xsd:anyURI .

C1901A00006:169 a legcons:Item,
        skos:Concept,
        dcat:Resource ;
    rdfs:label "Item I169"@en-AU ;
    rdfs:comment "71 K  Manner of communicating with Department by document - GraphNodeID: I169"@en-AU ;
    skos:definition "71 K  Manner of communicating with Department by document"@en-AU ;
    skos:narrower C1901A00006:163 ;
    skos:prefLabel "Item I169"@en-AU ;
    dcat:accessURL "https://www.legislation.gov.au/C1901A00006/2024-07-01/2024-07-01/text/original/epub/OEBPS/document_1/document_1.html#_Toc172623143"^^xsd:anyURI .

C1901A00006:17 a legcons:Item,
        skos:Concept,
        dcat:Resource ;
    rdfs:label "Item I17"@en-AU ;
    rdfs:comment "5 BA  Installation of overseas offshore electricity installations - GraphNodeID: I17"@en-AU ;
    skos:definition "5 BA  Installation of overseas offshore electricity installations"@en-AU ;
    skos:narrower C1901A00006:14 ;
    skos:prefLabel "Item I17"@en-AU ;
    dcat:accessURL "https://www.legislation.gov.au/C1901A00006/2024-07-01/2024-07-01/text/original/epub/OEBPS/document_1/document_1.html#_Toc172622991"^^xsd:anyURI .

C1901A00006:170 a legcons:Item,
        skos:Concept,
        dcat:Resource ;
    rdfs:label "Item I170"@en-AU ;
    rdfs:comment "71 L  Manner and effect of communicating with Department electronically - GraphNodeID: I170"@en-AU ;
    skos:definition "71 L  Manner and effect of communicating with Department electronically"@en-AU ;
    skos:narrower C1901A00006:163 ;
    skos:prefLabel "Item I170"@en-AU ;
    dcat:accessURL "https://www.legislation.gov.au/C1901A00006/2024-07-01/2024-07-01/text/original/epub/OEBPS/document_1/document_1.html#_Toc172623144"^^xsd:anyURI .

C1901A00006:171 a legcons:Item,
        skos:Concept,
        dcat:Resource ;
    rdfs:label "Item I171"@en-AU ;
    rdfs:comment "71 M  Requirements for communicating to Department electronically - GraphNodeID: I171"@en-AU ;
    skos:definition "71 M  Requirements for communicating to Department electronically"@en-AU ;
    skos:narrower C1901A00006:163 ;
    skos:prefLabel "Item I171"@en-AU ;
    dcat:accessURL "https://www.legislation.gov.au/C1901A00006/2024-07-01/2024-07-01/text/original/epub/OEBPS/document_1/document_1.html#_Toc172623145"^^xsd:anyURI .

C1901A00006:172 a legcons:Item,
        skos:Concept,
        dcat:Resource ;
    rdfs:label "Item I172"@en-AU ;
    rdfs:comment "72  Failure to make entries - GraphNodeID: I172"@en-AU ;
    skos:definition "72  Failure to make entries"@en-AU ;
    skos:narrower C1901A00006:163 ;
    skos:prefLabel "Item I172"@en-AU ;
    dcat:accessURL "https://www.legislation.gov.au/C1901A00006/2024-07-01/2024-07-01/text/original/epub/OEBPS/document_1/document_1.html#_Toc172623146"^^xsd:anyURI .

C1901A00006:173 a legcons:Item,
        skos:Concept,
        dcat:Resource ;
    rdfs:label "Item I173"@en-AU ;
    rdfs:comment "73  Breaking bulk - GraphNodeID: I173"@en-AU ;
    skos:definition "73  Breaking bulk"@en-AU ;
    skos:narrower C1901A00006:163 ;
    skos:prefLabel "Item I173"@en-AU ;
    dcat:accessURL "https://www.legislation.gov.au/C1901A00006/2024-07-01/2024-07-01/text/original/epub/OEBPS/document_1/document_1.html#_Toc172623147"^^xsd:anyURI .

C1901A00006:174 a legcons:Item,
        skos:Concept,
        dcat:Resource ;
    rdfs:label "Item I174"@en-AU ;
    rdfs:comment "74  Officer may give directions as to storage or movement of certain goods - GraphNodeID: I174"@en-AU ;
    skos:definition "74  Officer may give directions as to storage or movement of certain goods"@en-AU ;
    skos:narrower C1901A00006:163 ;
    skos:prefLabel "Item I174"@en-AU ;
    dcat:accessURL "https://www.legislation.gov.au/C1901A00006/2024-07-01/2024-07-01/text/original/epub/OEBPS/document_1/document_1.html#_Toc172623148"^^xsd:anyURI .

C1901A00006:175 a legcons:Item,
        skos:Concept,
        dcat:Resource ;
    rdfs:label "Item I175"@en-AU ;
    rdfs:comment "76  Goods landed at ships risk etc - GraphNodeID: I175"@en-AU ;
    skos:definition "76  Goods landed at ships risk etc"@en-AU ;
    skos:narrower C1901A00006:163 ;
    skos:prefLabel "Item I175"@en-AU ;
    dcat:accessURL "https://www.legislation.gov.au/C1901A00006/2024-07-01/2024-07-01/text/original/epub/OEBPS/document_1/document_1.html#_Toc172623149"^^xsd:anyURI .

C1901A00006:176 a legcons:Item,
        skos:Concept,
        dcat:Resource ;
    rdfs:label "Item I176"@en-AU ;
    rdfs:comment "77  Repacking on wharf - GraphNodeID: I176"@en-AU ;
    skos:definition "77  Repacking on wharf"@en-AU ;
    skos:narrower C1901A00006:163 ;
    skos:prefLabel "Item I176"@en-AU ;
    dcat:accessURL "https://www.legislation.gov.au/C1901A00006/2024-07-01/2024-07-01/text/original/epub/OEBPS/document_1/document_1.html#_Toc172623150"^^xsd:anyURI .

C1901A00006:177 a legcons:Item,
        skos:Concept,
        dcat:Resource ;
    rdfs:label "Item I177"@en-AU ;
    rdfs:comment "77 AA  Disclosure of information to cargo reporter or owner of goods - GraphNodeID: I177"@en-AU ;
    skos:definition "77 AA  Disclosure of information to cargo reporter or owner of goods"@en-AU ;
    skos:narrower C1901A00006:163 ;
    skos:prefLabel "Item I177"@en-AU ;
    dcat:accessURL "https://www.legislation.gov.au/C1901A00006/2024-07-01/2024-07-01/text/original/epub/OEBPS/document_1/document_1.html#_Toc172623151"^^xsd:anyURI .

C1901A00006:178 a legcons:Division,
        skos:Concept,
        dcat:Resource ;
    rdfs:label "Division D178"@en-AU ;
    rdfs:comment "Division 5 Detention of goods in the public interest - GraphNodeID: D178"@en-AU ;
    skos:definition "Division 5 Detention of goods in the public interest"@en-AU ;
    skos:narrower C1901A00006:54 ;
    skos:prefLabel "Division D178"@en-AU ;
    dcat:accessURL "https://www.legislation.gov.au/C1901A00006/2024-07-01/2024-07-01/text/original/epub/OEBPS/document_1/document_1.html#_Toc172623152"^^xsd:anyURI .

C1901A00006:179 a legcons:Item,
        skos:Concept,
        dcat:Resource ;
    rdfs:label "Item I179"@en-AU ;
    rdfs:comment "77 EA  Minister may order goods to be detained - GraphNodeID: I179"@en-AU ;
    skos:definition "77 EA  Minister may order goods to be detained"@en-AU ;
    skos:narrower C1901A00006:163 ;
    skos:prefLabel "Item I179"@en-AU ;
    dcat:accessURL "https://www.legislation.gov.au/C1901A00006/2024-07-01/2024-07-01/text/original/epub/OEBPS/document_1/document_1.html#_Toc172623153"^^xsd:anyURI .

C1901A00006:18 a legcons:Item,
        skos:Concept,
        dcat:Resource ;
    rdfs:label "Item I18"@en-AU ;
    rdfs:comment "5 C  Certain installations to be part of Australia - GraphNodeID: I18"@en-AU ;
    skos:definition "5 C  Certain installations to be part of Australia"@en-AU ;
    skos:narrower C1901A00006:14 ;
    skos:prefLabel "Item I18"@en-AU ;
    dcat:accessURL "https://www.legislation.gov.au/C1901A00006/2024-07-01/2024-07-01/text/original/epub/OEBPS/document_1/document_1.html#_Toc172622992"^^xsd:anyURI .

C1901A00006:180 a legcons:Item,
        skos:Concept,
        dcat:Resource ;
    rdfs:label "Item I180"@en-AU ;
    rdfs:comment "77 EB  Notice to person whose goods are detained - GraphNodeID: I180"@en-AU ;
    skos:definition "77 EB  Notice to person whose goods are detained"@en-AU ;
    skos:narrower C1901A00006:163 ;
    skos:prefLabel "Item I180"@en-AU ;
    dcat:accessURL "https://www.legislation.gov.au/C1901A00006/2024-07-01/2024-07-01/text/original/epub/OEBPS/document_1/document_1.html#_Toc172623154"^^xsd:anyURI .

C1901A00006:181 a legcons:Item,
        skos:Concept,
        dcat:Resource ;
    rdfs:label "Item I181"@en-AU ;
    rdfs:comment "77 EC  Detention of goods by Collector - GraphNodeID: I181"@en-AU ;
    skos:definition "77 EC  Detention of goods by Collector"@en-AU ;
    skos:narrower C1901A00006:163 ;
    skos:prefLabel "Item I181"@en-AU ;
    dcat:accessURL "https://www.legislation.gov.au/C1901A00006/2024-07-01/2024-07-01/text/original/epub/OEBPS/document_1/document_1.html#_Toc172623155"^^xsd:anyURI .

C1901A00006:182 a legcons:Item,
        skos:Concept,
        dcat:Resource ;
    rdfs:label "Item I182"@en-AU ;
    rdfs:comment "77 ED  Minister may authorise delivery of detained goods into home consumption - GraphNodeID: I182"@en-AU ;
    skos:definition "77 ED  Minister may authorise delivery of detained goods into home consumption"@en-AU ;
    skos:narrower C1901A00006:163 ;
    skos:prefLabel "Item I182"@en-AU ;
    dcat:accessURL "https://www.legislation.gov.au/C1901A00006/2024-07-01/2024-07-01/text/original/epub/OEBPS/document_1/document_1.html#_Toc172623156"^^xsd:anyURI .

C1901A00006:183 a legcons:Item,
        skos:Concept,
        dcat:Resource ;
    rdfs:label "Item I183"@en-AU ;
    rdfs:comment "77 EE  Minister may authorise export of detained goods - GraphNodeID: I183"@en-AU ;
    skos:definition "77 EE  Minister may authorise export of detained goods"@en-AU ;
    skos:narrower C1901A00006:163 ;
    skos:prefLabel "Item I183"@en-AU ;
    dcat:accessURL "https://www.legislation.gov.au/C1901A00006/2024-07-01/2024-07-01/text/original/epub/OEBPS/document_1/document_1.html#_Toc172623157"^^xsd:anyURI .

C1901A00006:184 a legcons:Item,
        skos:Concept,
        dcat:Resource ;
    rdfs:label "Item I184"@en-AU ;
    rdfs:comment "77 EF  When goods have been detained for 12 months - GraphNodeID: I184"@en-AU ;
    skos:definition "77 EF  When goods have been detained for 12 months"@en-AU ;
    skos:narrower C1901A00006:163 ;
    skos:prefLabel "Item I184"@en-AU ;
    dcat:accessURL "https://www.legislation.gov.au/C1901A00006/2024-07-01/2024-07-01/text/original/epub/OEBPS/document_1/document_1.html#_Toc172623158"^^xsd:anyURI .

C1901A00006:185 a legcons:Part,
        skos:Concept,
        dcat:Resource ;
    rdfs:label "Part P185"@en-AU ;
    rdfs:comment "Part IVADepots - GraphNodeID: P185"@en-AU ;
    skos:definition "Part IVADepots"@en-AU ;
    skos:narrower C1901A00006:1 ;
    skos:prefLabel "Part P185"@en-AU ;
    dcat:accessURL "https://www.legislation.gov.au/C1901A00006/2024-07-01/2024-07-01/text/original/epub/OEBPS/document_1/document_1.html#_Toc172623159"^^xsd:anyURI .

C1901A00006:186 a legcons:Item,
        skos:Concept,
        dcat:Resource ;
    rdfs:label "Item I186"@en-AU ;
    rdfs:comment "77 F  Interpretation - GraphNodeID: I186"@en-AU ;
    skos:definition "77 F  Interpretation"@en-AU ;
    skos:narrower C1901A00006:163 ;
    skos:prefLabel "Item I186"@en-AU ;
    dcat:accessURL "https://www.legislation.gov.au/C1901A00006/2024-07-01/2024-07-01/text/original/epub/OEBPS/document_1/document_1.html#_Toc172623160"^^xsd:anyURI .

C1901A00006:187 a legcons:Item,
        skos:Concept,
        dcat:Resource ;
    rdfs:label "Item I187"@en-AU ;
    rdfs:comment "77 G  Depot licences - GraphNodeID: I187"@en-AU ;
    skos:definition "77 G  Depot licences"@en-AU ;
    skos:narrower C1901A00006:163 ;
    skos:prefLabel "Item I187"@en-AU ;
    dcat:accessURL "https://www.legislation.gov.au/C1901A00006/2024-07-01/2024-07-01/text/original/epub/OEBPS/document_1/document_1.html#_Toc172623161"^^xsd:anyURI .

C1901A00006:188 a legcons:Item,
        skos:Concept,
        dcat:Resource ;
    rdfs:label "Item I188"@en-AU ;
    rdfs:comment "77 H  Application for a depot licence - GraphNodeID: I188"@en-AU ;
    skos:definition "77 H  Application for a depot licence"@en-AU ;
    skos:narrower C1901A00006:163 ;
    skos:prefLabel "Item I188"@en-AU ;
    dcat:accessURL "https://www.legislation.gov.au/C1901A00006/2024-07-01/2024-07-01/text/original/epub/OEBPS/document_1/document_1.html#_Toc172623162"^^xsd:anyURI .

C1901A00006:189 a legcons:Item,
        skos:Concept,
        dcat:Resource ;
    rdfs:label "Item I189"@en-AU ;
    rdfs:comment "77 J  Comptroller General of Customs may require applicant to supply further information - GraphNodeID: I189"@en-AU ;
    skos:definition "77 J  Comptroller General of Customs may require applicant to supply further information"@en-AU ;
    skos:narrower C1901A00006:163 ;
    skos:prefLabel "Item I189"@en-AU ;
    dcat:accessURL "https://www.legislation.gov.au/C1901A00006/2024-07-01/2024-07-01/text/original/epub/OEBPS/document_1/document_1.html#_Toc172623163"^^xsd:anyURI .

C1901A00006:19 a legcons:Item,
        skos:Concept,
        dcat:Resource ;
    rdfs:label "Item I19"@en-AU ;
    rdfs:comment "6  Act does not extend to external Territories - GraphNodeID: I19"@en-AU ;
    skos:definition "6  Act does not extend to external Territories"@en-AU ;
    skos:narrower C1901A00006:14 ;
    skos:prefLabel "Item I19"@en-AU ;
    dcat:accessURL "https://www.legislation.gov.au/C1901A00006/2024-07-01/2024-07-01/text/original/epub/OEBPS/document_1/document_1.html#_Toc172622993"^^xsd:anyURI .

C1901A00006:190 a legcons:Item,
        skos:Concept,
        dcat:Resource ;
    rdfs:label "Item I190"@en-AU ;
    rdfs:comment "77 K  Requirements for grant of depot licence - GraphNodeID: I190"@en-AU ;
    skos:definition "77 K  Requirements for grant of depot licence"@en-AU ;
    skos:narrower C1901A00006:163 ;
    skos:prefLabel "Item I190"@en-AU ;
    dcat:accessURL "https://www.legislation.gov.au/C1901A00006/2024-07-01/2024-07-01/text/original/epub/OEBPS/document_1/document_1.html#_Toc172623164"^^xsd:anyURI .

C1901A00006:191 a legcons:Item,
        skos:Concept,
        dcat:Resource ;
    rdfs:label "Item I191"@en-AU ;
    rdfs:comment "77 L  Granting of a depot licence - GraphNodeID: I191"@en-AU ;
    skos:definition "77 L  Granting of a depot licence"@en-AU ;
    skos:narrower C1901A00006:163 ;
    skos:prefLabel "Item I191"@en-AU ;
    dcat:accessURL "https://www.legislation.gov.au/C1901A00006/2024-07-01/2024-07-01/text/original/epub/OEBPS/document_1/document_1.html#_Toc172623165"^^xsd:anyURI .

C1901A00006:192 a legcons:Item,
        skos:Concept,
        dcat:Resource ;
    rdfs:label "Item I192"@en-AU ;
    rdfs:comment "77 LA  Variation of places covered by depot licence - GraphNodeID: I192"@en-AU ;
    skos:definition "77 LA  Variation of places covered by depot licence"@en-AU ;
    skos:narrower C1901A00006:163 ;
    skos:prefLabel "Item I192"@en-AU ;
    dcat:accessURL "https://www.legislation.gov.au/C1901A00006/2024-07-01/2024-07-01/text/original/epub/OEBPS/document_1/document_1.html#_Toc172623166"^^xsd:anyURI .

C1901A00006:193 a legcons:Item,
        skos:Concept,
        dcat:Resource ;
    rdfs:label "Item I193"@en-AU ;
    rdfs:comment "77 N  Conditions of a depot licencegeneral - GraphNodeID: I193"@en-AU ;
    skos:definition "77 N  Conditions of a depot licencegeneral"@en-AU ;
    skos:narrower C1901A00006:163 ;
    skos:prefLabel "Item I193"@en-AU ;
    dcat:accessURL "https://www.legislation.gov.au/C1901A00006/2024-07-01/2024-07-01/text/original/epub/OEBPS/document_1/document_1.html#_Toc172623167"^^xsd:anyURI .

C1901A00006:194 a legcons:Item,
        skos:Concept,
        dcat:Resource ;
    rdfs:label "Item I194"@en-AU ;
    rdfs:comment "77 P  Conditions of a depot licenceimported goods - GraphNodeID: I194"@en-AU ;
    skos:definition "77 P  Conditions of a depot licenceimported goods"@en-AU ;
    skos:narrower C1901A00006:163 ;
    skos:prefLabel "Item I194"@en-AU ;
    dcat:accessURL "https://www.legislation.gov.au/C1901A00006/2024-07-01/2024-07-01/text/original/epub/OEBPS/document_1/document_1.html#_Toc172623168"^^xsd:anyURI .

C1901A00006:195 a legcons:Item,
        skos:Concept,
        dcat:Resource ;
    rdfs:label "Item I195"@en-AU ;
    rdfs:comment "77 Q  Comptroller General of Customs may impose additional conditions to which a depot licence is subject - GraphNodeID: I195"@en-AU ;
    skos:definition "77 Q  Comptroller General of Customs may impose additional conditions to which a depot licence is subject"@en-AU ;
    skos:narrower C1901A00006:163 ;
    skos:prefLabel "Item I195"@en-AU ;
    dcat:accessURL "https://www.legislation.gov.au/C1901A00006/2024-07-01/2024-07-01/text/original/epub/OEBPS/document_1/document_1.html#_Toc172623169"^^xsd:anyURI .

C1901A00006:196 a legcons:Item,
        skos:Concept,
        dcat:Resource ;
    rdfs:label "Item I196"@en-AU ;
    rdfs:comment "77 R  Breach of conditions of depot licence - GraphNodeID: I196"@en-AU ;
    skos:definition "77 R  Breach of conditions of depot licence"@en-AU ;
    skos:narrower C1901A00006:163 ;
    skos:prefLabel "Item I196"@en-AU ;
    dcat:accessURL "https://www.legislation.gov.au/C1901A00006/2024-07-01/2024-07-01/text/original/epub/OEBPS/document_1/document_1.html#_Toc172623170"^^xsd:anyURI .

C1901A00006:197 a legcons:Item,
        skos:Concept,
        dcat:Resource ;
    rdfs:label "Item I197"@en-AU ;
    rdfs:comment "77 S  Duration of depot licences - GraphNodeID: I197"@en-AU ;
    skos:definition "77 S  Duration of depot licences"@en-AU ;
    skos:narrower C1901A00006:163 ;
    skos:prefLabel "Item I197"@en-AU ;
    dcat:accessURL "https://www.legislation.gov.au/C1901A00006/2024-07-01/2024-07-01/text/original/epub/OEBPS/document_1/document_1.html#_Toc172623171"^^xsd:anyURI .

C1901A00006:198 a legcons:Item,
        skos:Concept,
        dcat:Resource ;
    rdfs:label "Item I198"@en-AU ;
    rdfs:comment "77 T  Renewal of depot licences - GraphNodeID: I198"@en-AU ;
    skos:definition "77 T  Renewal of depot licences"@en-AU ;
    skos:narrower C1901A00006:163 ;
    skos:prefLabel "Item I198"@en-AU ;
    dcat:accessURL "https://www.legislation.gov.au/C1901A00006/2024-07-01/2024-07-01/text/original/epub/OEBPS/document_1/document_1.html#_Toc172623172"^^xsd:anyURI .

C1901A00006:199 a legcons:Item,
        skos:Concept,
        dcat:Resource ;
    rdfs:label "Item I199"@en-AU ;
    rdfs:comment "77 U  Licence charges - GraphNodeID: I199"@en-AU ;
    skos:definition "77 U  Licence charges"@en-AU ;
    skos:narrower C1901A00006:163 ;
    skos:prefLabel "Item I199"@en-AU ;
    dcat:accessURL "https://www.legislation.gov.au/C1901A00006/2024-07-01/2024-07-01/text/original/epub/OEBPS/document_1/document_1.html#_Toc172623173"^^xsd:anyURI .

C1901A00006:20 a legcons:Item,
        skos:Concept,
        dcat:Resource ;
    rdfs:label "Item I20"@en-AU ;
    rdfs:comment "7  General administration of Act - GraphNodeID: I20"@en-AU ;
    skos:definition "7  General administration of Act"@en-AU ;
    skos:narrower C1901A00006:14 ;
    skos:prefLabel "Item I20"@en-AU ;
    dcat:accessURL "https://www.legislation.gov.au/C1901A00006/2024-07-01/2024-07-01/text/original/epub/OEBPS/document_1/document_1.html#_Toc172622994"^^xsd:anyURI .

C1901A00006:200 a legcons:Item,
        skos:Concept,
        dcat:Resource ;
    rdfs:label "Item I200"@en-AU ;
    rdfs:comment "77 V  Notice of intended cancellation etc of a depot licence - GraphNodeID: I200"@en-AU ;
    skos:definition "77 V  Notice of intended cancellation etc of a depot licence"@en-AU ;
    skos:narrower C1901A00006:163 ;
    skos:prefLabel "Item I200"@en-AU ;
    dcat:accessURL "https://www.legislation.gov.au/C1901A00006/2024-07-01/2024-07-01/text/original/epub/OEBPS/document_1/document_1.html#_Toc172623174"^^xsd:anyURI .

C1901A00006:201 a legcons:Item,
        skos:Concept,
        dcat:Resource ;
    rdfs:label "Item I201"@en-AU ;
    rdfs:comment "77 VA  Depot must not be used if depot licence is suspended etc - GraphNodeID: I201"@en-AU ;
    skos:definition "77 VA  Depot must not be used if depot licence is suspended etc"@en-AU ;
    skos:narrower C1901A00006:163 ;
    skos:prefLabel "Item I201"@en-AU ;
    dcat:accessURL "https://www.legislation.gov.au/C1901A00006/2024-07-01/2024-07-01/text/original/epub/OEBPS/document_1/document_1.html#_Toc172623175"^^xsd:anyURI .

C1901A00006:202 a legcons:Item,
        skos:Concept,
        dcat:Resource ;
    rdfs:label "Item I202"@en-AU ;
    rdfs:comment "77 VB  Revocation of suspension of depot licences - GraphNodeID: I202"@en-AU ;
    skos:definition "77 VB  Revocation of suspension of depot licences"@en-AU ;
    skos:narrower C1901A00006:163 ;
    skos:prefLabel "Item I202"@en-AU ;
    dcat:accessURL "https://www.legislation.gov.au/C1901A00006/2024-07-01/2024-07-01/text/original/epub/OEBPS/document_1/document_1.html#_Toc172623176"^^xsd:anyURI .

C1901A00006:203 a legcons:Item,
        skos:Concept,
        dcat:Resource ;
    rdfs:label "Item I203"@en-AU ;
    rdfs:comment "77 VC  Cancellation of depot licences - GraphNodeID: I203"@en-AU ;
    skos:definition "77 VC  Cancellation of depot licences"@en-AU ;
    skos:narrower C1901A00006:163 ;
    skos:prefLabel "Item I203"@en-AU ;
    dcat:accessURL "https://www.legislation.gov.au/C1901A00006/2024-07-01/2024-07-01/text/original/epub/OEBPS/document_1/document_1.html#_Toc172623177"^^xsd:anyURI .

C1901A00006:204 a legcons:Item,
        skos:Concept,
        dcat:Resource ;
    rdfs:label "Item I204"@en-AU ;
    rdfs:comment "77 W  Refund of depot licence charge on cancellation of a depot licence - GraphNodeID: I204"@en-AU ;
    skos:definition "77 W  Refund of depot licence charge on cancellation of a depot licence"@en-AU ;
    skos:narrower C1901A00006:163 ;
    skos:prefLabel "Item I204"@en-AU ;
    dcat:accessURL "https://www.legislation.gov.au/C1901A00006/2024-07-01/2024-07-01/text/original/epub/OEBPS/document_1/document_1.html#_Toc172623178"^^xsd:anyURI .

C1901A00006:205 a legcons:Item,
        skos:Concept,
        dcat:Resource ;
    rdfs:label "Item I205"@en-AU ;
    rdfs:comment "77 X  Collectors powers in relation to a place that is no longer a depot - GraphNodeID: I205"@en-AU ;
    skos:definition "77 X  Collectors powers in relation to a place that is no longer a depot"@en-AU ;
    skos:narrower C1901A00006:163 ;
    skos:prefLabel "Item I205"@en-AU ;
    dcat:accessURL "https://www.legislation.gov.au/C1901A00006/2024-07-01/2024-07-01/text/original/epub/OEBPS/document_1/document_1.html#_Toc172623179"^^xsd:anyURI .

C1901A00006:206 a legcons:Item,
        skos:Concept,
        dcat:Resource ;
    rdfs:label "Item I206"@en-AU ;
    rdfs:comment "77 Y  Collector may give directions in relation to goods subject to customs control - GraphNodeID: I206"@en-AU ;
    skos:definition "77 Y  Collector may give directions in relation to goods subject to customs control"@en-AU ;
    skos:narrower C1901A00006:163 ;
    skos:prefLabel "Item I206"@en-AU ;
    dcat:accessURL "https://www.legislation.gov.au/C1901A00006/2024-07-01/2024-07-01/text/original/epub/OEBPS/document_1/document_1.html#_Toc172623180"^^xsd:anyURI .

C1901A00006:207 a legcons:Item,
        skos:Concept,
        dcat:Resource ;
    rdfs:label "Item I207"@en-AU ;
    rdfs:comment "77 Z  Licences cannot be transferred - GraphNodeID: I207"@en-AU ;
    skos:definition "77 Z  Licences cannot be transferred"@en-AU ;
    skos:narrower C1901A00006:163 ;
    skos:prefLabel "Item I207"@en-AU ;
    dcat:accessURL "https://www.legislation.gov.au/C1901A00006/2024-07-01/2024-07-01/text/original/epub/OEBPS/document_1/document_1.html#_Toc172623181"^^xsd:anyURI .

C1901A00006:208 a legcons:Item,
        skos:Concept,
        dcat:Resource ;
    rdfs:label "Item I208"@en-AU ;
    rdfs:comment "77 ZA  Service of notice - GraphNodeID: I208"@en-AU ;
    skos:definition "77 ZA  Service of notice"@en-AU ;
    skos:narrower C1901A00006:163 ;
    skos:prefLabel "Item I208"@en-AU ;
    dcat:accessURL "https://www.legislation.gov.au/C1901A00006/2024-07-01/2024-07-01/text/original/epub/OEBPS/document_1/document_1.html#_Toc172623182"^^xsd:anyURI .

C1901A00006:209 a legcons:Part,
        skos:Concept,
        dcat:Resource ;
    rdfs:label "Part P209"@en-AU ;
    rdfs:comment "Part VWarehouses - GraphNodeID: P209"@en-AU ;
    skos:definition "Part VWarehouses"@en-AU ;
    skos:narrower C1901A00006:1 ;
    skos:prefLabel "Part P209"@en-AU ;
    dcat:accessURL "https://www.legislation.gov.au/C1901A00006/2024-07-01/2024-07-01/text/original/epub/OEBPS/document_1/document_1.html#_Toc172623183"^^xsd:anyURI .

C1901A00006:21 a legcons:Item,
        skos:Concept,
        dcat:Resource ;
    rdfs:label "Item I21"@en-AU ;
    rdfs:comment "8  Collectors States and Northern Territory - GraphNodeID: I21"@en-AU ;
    skos:definition "8  Collectors States and Northern Territory"@en-AU ;
    skos:narrower C1901A00006:14 ;
    skos:prefLabel "Item I21"@en-AU ;
    dcat:accessURL "https://www.legislation.gov.au/C1901A00006/2024-07-01/2024-07-01/text/original/epub/OEBPS/document_1/document_1.html#_Toc172622995"^^xsd:anyURI .

C1901A00006:210 a legcons:Item,
        skos:Concept,
        dcat:Resource ;
    rdfs:label "Item I210"@en-AU ;
    rdfs:comment "78  Interpretation - GraphNodeID: I210"@en-AU ;
    skos:definition "78  Interpretation"@en-AU ;
    skos:narrower C1901A00006:163 ;
    skos:prefLabel "Item I210"@en-AU ;
    dcat:accessURL "https://www.legislation.gov.au/C1901A00006/2024-07-01/2024-07-01/text/original/epub/OEBPS/document_1/document_1.html#_Toc172623184"^^xsd:anyURI .

C1901A00006:211 a legcons:Item,
        skos:Concept,
        dcat:Resource ;
    rdfs:label "Item I211"@en-AU ;
    rdfs:comment "79  Warehouse licences - GraphNodeID: I211"@en-AU ;
    skos:definition "79  Warehouse licences"@en-AU ;
    skos:narrower C1901A00006:163 ;
    skos:prefLabel "Item I211"@en-AU ;
    dcat:accessURL "https://www.legislation.gov.au/C1901A00006/2024-07-01/2024-07-01/text/original/epub/OEBPS/document_1/document_1.html#_Toc172623185"^^xsd:anyURI .

C1901A00006:212 a legcons:Item,
        skos:Concept,
        dcat:Resource ;
    rdfs:label "Item I212"@en-AU ;
    rdfs:comment "80  Applications for warehouse licences - GraphNodeID: I212"@en-AU ;
    skos:definition "80  Applications for warehouse licences"@en-AU ;
    skos:narrower C1901A00006:163 ;
    skos:prefLabel "Item I212"@en-AU ;
    dcat:accessURL "https://www.legislation.gov.au/C1901A00006/2024-07-01/2024-07-01/text/original/epub/OEBPS/document_1/document_1.html#_Toc172623186"^^xsd:anyURI .

C1901A00006:213 a legcons:Item,
        skos:Concept,
        dcat:Resource ;
    rdfs:label "Item I213"@en-AU ;
    rdfs:comment "80 A  Comptroller General of Customs may require applicant to supply further information - GraphNodeID: I213"@en-AU ;
    skos:definition "80 A  Comptroller General of Customs may require applicant to supply further information"@en-AU ;
    skos:narrower C1901A00006:163 ;
    skos:prefLabel "Item I213"@en-AU ;
    dcat:accessURL "https://www.legislation.gov.au/C1901A00006/2024-07-01/2024-07-01/text/original/epub/OEBPS/document_1/document_1.html#_Toc172623187"^^xsd:anyURI .

C1901A00006:214 a legcons:Item,
        skos:Concept,
        dcat:Resource ;
    rdfs:label "Item I214"@en-AU ;
    rdfs:comment "81  Requirements for grant of warehouse licence - GraphNodeID: I214"@en-AU ;
    skos:definition "81  Requirements for grant of warehouse licence"@en-AU ;
    skos:narrower C1901A00006:163 ;
    skos:prefLabel "Item I214"@en-AU ;
    dcat:accessURL "https://www.legislation.gov.au/C1901A00006/2024-07-01/2024-07-01/text/original/epub/OEBPS/document_1/document_1.html#_Toc172623188"^^xsd:anyURI .

C1901A00006:215 a legcons:Item,
        skos:Concept,
        dcat:Resource ;
    rdfs:label "Item I215"@en-AU ;
    rdfs:comment "81 A  Grant of a warehouse licence - GraphNodeID: I215"@en-AU ;
    skos:definition "81 A  Grant of a warehouse licence"@en-AU ;
    skos:narrower C1901A00006:163 ;
    skos:prefLabel "Item I215"@en-AU ;
    dcat:accessURL "https://www.legislation.gov.au/C1901A00006/2024-07-01/2024-07-01/text/original/epub/OEBPS/document_1/document_1.html#_Toc172623189"^^xsd:anyURI .

C1901A00006:216 a legcons:Item,
        skos:Concept,
        dcat:Resource ;
    rdfs:label "Item I216"@en-AU ;
    rdfs:comment "81 B  Variation of the place covered by a warehouse licence - GraphNodeID: I216"@en-AU ;
    skos:definition "81 B  Variation of the place covered by a warehouse licence"@en-AU ;
    skos:narrower C1901A00006:163 ;
    skos:prefLabel "Item I216"@en-AU ;
    dcat:accessURL "https://www.legislation.gov.au/C1901A00006/2024-07-01/2024-07-01/text/original/epub/OEBPS/document_1/document_1.html#_Toc172623190"^^xsd:anyURI .

C1901A00006:217 a legcons:Item,
        skos:Concept,
        dcat:Resource ;
    rdfs:label "Item I217"@en-AU ;
    rdfs:comment "82  Conditions of warehouse licences - GraphNodeID: I217"@en-AU ;
    skos:definition "82  Conditions of warehouse licences"@en-AU ;
    skos:narrower C1901A00006:163 ;
    skos:prefLabel "Item I217"@en-AU ;
    dcat:accessURL "https://www.legislation.gov.au/C1901A00006/2024-07-01/2024-07-01/text/original/epub/OEBPS/document_1/document_1.html#_Toc172623191"^^xsd:anyURI .

C1901A00006:218 a legcons:Item,
        skos:Concept,
        dcat:Resource ;
    rdfs:label "Item I218"@en-AU ;
    rdfs:comment "82 A  Comptroller General of Customs may impose additional conditions to which a warehouse licence is subject - GraphNodeID: I218"@en-AU ;
    skos:definition "82 A  Comptroller General of Customs may impose additional conditions to which a warehouse licence is subject"@en-AU ;
    skos:narrower C1901A00006:163 ;
    skos:prefLabel "Item I218"@en-AU ;
    dcat:accessURL "https://www.legislation.gov.au/C1901A00006/2024-07-01/2024-07-01/text/original/epub/OEBPS/document_1/document_1.html#_Toc172623192"^^xsd:anyURI .

C1901A00006:219 a legcons:Item,
        skos:Concept,
        dcat:Resource ;
    rdfs:label "Item I219"@en-AU ;
    rdfs:comment "82 B  Comptroller General of Customs may vary the conditions to which a warehouse licence is subject - GraphNodeID: I219"@en-AU ;
    skos:definition "82 B  Comptroller General of Customs may vary the conditions to which a warehouse licence is subject"@en-AU ;
    skos:narrower C1901A00006:163 ;
    skos:prefLabel "Item I219"@en-AU ;
    dcat:accessURL "https://www.legislation.gov.au/C1901A00006/2024-07-01/2024-07-01/text/original/epub/OEBPS/document_1/document_1.html#_Toc172623193"^^xsd:anyURI .

C1901A00006:22 a legcons:Item,
        skos:Concept,
        dcat:Resource ;
    rdfs:label "Item I22"@en-AU ;
    rdfs:comment "8 A  Attachment of part of a State or Territory to adjoining State or Territory for administrative purposes - GraphNodeID: I22"@en-AU ;
    skos:definition "8 A  Attachment of part of a State or Territory to adjoining State or Territory for administrative purposes"@en-AU ;
    skos:narrower C1901A00006:14 ;
    skos:prefLabel "Item I22"@en-AU ;
    dcat:accessURL "https://www.legislation.gov.au/C1901A00006/2024-07-01/2024-07-01/text/original/epub/OEBPS/document_1/document_1.html#_Toc172622996"^^xsd:anyURI .

C1901A00006:220 a legcons:Item,
        skos:Concept,
        dcat:Resource ;
    rdfs:label "Item I220"@en-AU ;
    rdfs:comment "82 C  Breach of conditions of a warehouse licence - GraphNodeID: I220"@en-AU ;
    skos:definition "82 C  Breach of conditions of a warehouse licence"@en-AU ;
    skos:narrower C1901A00006:163 ;
    skos:prefLabel "Item I220"@en-AU ;
    dcat:accessURL "https://www.legislation.gov.au/C1901A00006/2024-07-01/2024-07-01/text/original/epub/OEBPS/document_1/document_1.html#_Toc172623194"^^xsd:anyURI .

C1901A00006:221 a legcons:Item,
        skos:Concept,
        dcat:Resource ;
    rdfs:label "Item I221"@en-AU ;
    rdfs:comment "83  Duration of warehouse licence - GraphNodeID: I221"@en-AU ;
    skos:definition "83  Duration of warehouse licence"@en-AU ;
    skos:narrower C1901A00006:163 ;
    skos:prefLabel "Item I221"@en-AU ;
    dcat:accessURL "https://www.legislation.gov.au/C1901A00006/2024-07-01/2024-07-01/text/original/epub/OEBPS/document_1/document_1.html#_Toc172623195"^^xsd:anyURI .

C1901A00006:222 a legcons:Item,
        skos:Concept,
        dcat:Resource ;
    rdfs:label "Item I222"@en-AU ;
    rdfs:comment "84  Renewal of warehouse licence - GraphNodeID: I222"@en-AU ;
    skos:definition "84  Renewal of warehouse licence"@en-AU ;
    skos:narrower C1901A00006:163 ;
    skos:prefLabel "Item I222"@en-AU ;
    dcat:accessURL "https://www.legislation.gov.au/C1901A00006/2024-07-01/2024-07-01/text/original/epub/OEBPS/document_1/document_1.html#_Toc172623196"^^xsd:anyURI .

C1901A00006:223 a legcons:Item,
        skos:Concept,
        dcat:Resource ;
    rdfs:label "Item I223"@en-AU ;
    rdfs:comment "85  Licence charges - GraphNodeID: I223"@en-AU ;
    skos:definition "85  Licence charges"@en-AU ;
    skos:narrower C1901A00006:163 ;
    skos:prefLabel "Item I223"@en-AU ;
    dcat:accessURL "https://www.legislation.gov.au/C1901A00006/2024-07-01/2024-07-01/text/original/epub/OEBPS/document_1/document_1.html#_Toc172623197"^^xsd:anyURI .

C1901A00006:224 a legcons:Item,
        skos:Concept,
        dcat:Resource ;
    rdfs:label "Item I224"@en-AU ;
    rdfs:comment "85 A  Payment of warehouse licence charge - GraphNodeID: I224"@en-AU ;
    skos:definition "85 A  Payment of warehouse licence charge"@en-AU ;
    skos:narrower C1901A00006:163 ;
    skos:prefLabel "Item I224"@en-AU ;
    dcat:accessURL "https://www.legislation.gov.au/C1901A00006/2024-07-01/2024-07-01/text/original/epub/OEBPS/document_1/document_1.html#_Toc172623198"^^xsd:anyURI .

C1901A00006:225 a legcons:Item,
        skos:Concept,
        dcat:Resource ;
    rdfs:label "Item I225"@en-AU ;
    rdfs:comment "86  Suspension of warehouse licences - GraphNodeID: I225"@en-AU ;
    skos:definition "86  Suspension of warehouse licences"@en-AU ;
    skos:narrower C1901A00006:163 ;
    skos:prefLabel "Item I225"@en-AU ;
    dcat:accessURL "https://www.legislation.gov.au/C1901A00006/2024-07-01/2024-07-01/text/original/epub/OEBPS/document_1/document_1.html#_Toc172623199"^^xsd:anyURI .

C1901A00006:226 a legcons:Item,
        skos:Concept,
        dcat:Resource ;
    rdfs:label "Item I226"@en-AU ;
    rdfs:comment "87  Cancellation of warehouse licences - GraphNodeID: I226"@en-AU ;
    skos:definition "87  Cancellation of warehouse licences"@en-AU ;
    skos:narrower C1901A00006:163 ;
    skos:prefLabel "Item I226"@en-AU ;
    dcat:accessURL "https://www.legislation.gov.au/C1901A00006/2024-07-01/2024-07-01/text/original/epub/OEBPS/document_1/document_1.html#_Toc172623200"^^xsd:anyURI .

C1901A00006:227 a legcons:Item,
        skos:Concept,
        dcat:Resource ;
    rdfs:label "Item I227"@en-AU ;
    rdfs:comment "87 A  Refund of warehouse licence charge - GraphNodeID: I227"@en-AU ;
    skos:definition "87 A  Refund of warehouse licence charge"@en-AU ;
    skos:narrower C1901A00006:163 ;
    skos:prefLabel "Item I227"@en-AU ;
    dcat:accessURL "https://www.legislation.gov.au/C1901A00006/2024-07-01/2024-07-01/text/original/epub/OEBPS/document_1/document_1.html#_Toc172623201"^^xsd:anyURI .

C1901A00006:228 a legcons:Item,
        skos:Concept,
        dcat:Resource ;
    rdfs:label "Item I228"@en-AU ;
    rdfs:comment "87 B  Variation of excise equivalent warehouse licence to remove warehouse - GraphNodeID: I228"@en-AU ;
    skos:definition "87 B  Variation of excise equivalent warehouse licence to remove warehouse"@en-AU ;
    skos:narrower C1901A00006:163 ;
    skos:prefLabel "Item I228"@en-AU ;
    dcat:accessURL "https://www.legislation.gov.au/C1901A00006/2024-07-01/2024-07-01/text/original/epub/OEBPS/document_1/document_1.html#_Toc172623202"^^xsd:anyURI .

C1901A00006:229 a legcons:Item,
        skos:Concept,
        dcat:Resource ;
    rdfs:label "Item I229"@en-AU ;
    rdfs:comment "88  Service of notices - GraphNodeID: I229"@en-AU ;
    skos:definition "88  Service of notices"@en-AU ;
    skos:narrower C1901A00006:163 ;
    skos:prefLabel "Item I229"@en-AU ;
    dcat:accessURL "https://www.legislation.gov.au/C1901A00006/2024-07-01/2024-07-01/text/original/epub/OEBPS/document_1/document_1.html#_Toc172623203"^^xsd:anyURI .

C1901A00006:23 a legcons:Item,
        skos:Concept,
        dcat:Resource ;
    rdfs:label "Item I23"@en-AU ;
    rdfs:comment "9  Delegation - GraphNodeID: I23"@en-AU ;
    skos:definition "9  Delegation"@en-AU ;
    skos:narrower C1901A00006:14 ;
    skos:prefLabel "Item I23"@en-AU ;
    dcat:accessURL "https://www.legislation.gov.au/C1901A00006/2024-07-01/2024-07-01/text/original/epub/OEBPS/document_1/document_1.html#_Toc172622997"^^xsd:anyURI .

C1901A00006:230 a legcons:Item,
        skos:Concept,
        dcat:Resource ;
    rdfs:label "Item I230"@en-AU ;
    rdfs:comment "89  Death of licence holder - GraphNodeID: I230"@en-AU ;
    skos:definition "89  Death of licence holder"@en-AU ;
    skos:narrower C1901A00006:163 ;
    skos:prefLabel "Item I230"@en-AU ;
    dcat:accessURL "https://www.legislation.gov.au/C1901A00006/2024-07-01/2024-07-01/text/original/epub/OEBPS/document_1/document_1.html#_Toc172623204"^^xsd:anyURI .

C1901A00006:231 a legcons:Item,
        skos:Concept,
        dcat:Resource ;
    rdfs:label "Item I231"@en-AU ;
    rdfs:comment "90  Obligations of holders of warehouse licences - GraphNodeID: I231"@en-AU ;
    skos:definition "90  Obligations of holders of warehouse licences"@en-AU ;
    skos:narrower C1901A00006:163 ;
    skos:prefLabel "Item I231"@en-AU ;
    dcat:accessURL "https://www.legislation.gov.au/C1901A00006/2024-07-01/2024-07-01/text/original/epub/OEBPS/document_1/document_1.html#_Toc172623205"^^xsd:anyURI .

C1901A00006:232 a legcons:Item,
        skos:Concept,
        dcat:Resource ;
    rdfs:label "Item I232"@en-AU ;
    rdfs:comment "91  Access to warehouses - GraphNodeID: I232"@en-AU ;
    skos:definition "91  Access to warehouses"@en-AU ;
    skos:narrower C1901A00006:163 ;
    skos:prefLabel "Item I232"@en-AU ;
    dcat:accessURL "https://www.legislation.gov.au/C1901A00006/2024-07-01/2024-07-01/text/original/epub/OEBPS/document_1/document_1.html#_Toc172623206"^^xsd:anyURI .

C1901A00006:233 a legcons:Item,
        skos:Concept,
        dcat:Resource ;
    rdfs:label "Item I233"@en-AU ;
    rdfs:comment "92  Repacking in warehouse - GraphNodeID: I233"@en-AU ;
    skos:definition "92  Repacking in warehouse"@en-AU ;
    skos:narrower C1901A00006:163 ;
    skos:prefLabel "Item I233"@en-AU ;
    dcat:accessURL "https://www.legislation.gov.au/C1901A00006/2024-07-01/2024-07-01/text/original/epub/OEBPS/document_1/document_1.html#_Toc172623207"^^xsd:anyURI .

C1901A00006:234 a legcons:Item,
        skos:Concept,
        dcat:Resource ;
    rdfs:label "Item I234"@en-AU ;
    rdfs:comment "93  Regauging etc of goods - GraphNodeID: I234"@en-AU ;
    skos:definition "93  Regauging etc of goods"@en-AU ;
    skos:narrower C1901A00006:163 ;
    skos:prefLabel "Item I234"@en-AU ;
    dcat:accessURL "https://www.legislation.gov.au/C1901A00006/2024-07-01/2024-07-01/text/original/epub/OEBPS/document_1/document_1.html#_Toc172623208"^^xsd:anyURI .

C1901A00006:235 a legcons:Item,
        skos:Concept,
        dcat:Resource ;
    rdfs:label "Item I235"@en-AU ;
    rdfs:comment "94  Goods not worth duty may be destroyed - GraphNodeID: I235"@en-AU ;
    skos:definition "94  Goods not worth duty may be destroyed"@en-AU ;
    skos:narrower C1901A00006:163 ;
    skos:prefLabel "Item I235"@en-AU ;
    dcat:accessURL "https://www.legislation.gov.au/C1901A00006/2024-07-01/2024-07-01/text/original/epub/OEBPS/document_1/document_1.html#_Toc172623209"^^xsd:anyURI .

C1901A00006:236 a legcons:Item,
        skos:Concept,
        dcat:Resource ;
    rdfs:label "Item I236"@en-AU ;
    rdfs:comment "95  Revaluation - GraphNodeID: I236"@en-AU ;
    skos:definition "95  Revaluation"@en-AU ;
    skos:narrower C1901A00006:163 ;
    skos:prefLabel "Item I236"@en-AU ;
    dcat:accessURL "https://www.legislation.gov.au/C1901A00006/2024-07-01/2024-07-01/text/original/epub/OEBPS/document_1/document_1.html#_Toc172623210"^^xsd:anyURI .

C1901A00006:237 a legcons:Item,
        skos:Concept,
        dcat:Resource ;
    rdfs:label "Item I237"@en-AU ;
    rdfs:comment "96  Arrears of warehouse charges - GraphNodeID: I237"@en-AU ;
    skos:definition "96  Arrears of warehouse charges"@en-AU ;
    skos:narrower C1901A00006:163 ;
    skos:prefLabel "Item I237"@en-AU ;
    dcat:accessURL "https://www.legislation.gov.au/C1901A00006/2024-07-01/2024-07-01/text/original/epub/OEBPS/document_1/document_1.html#_Toc172623211"^^xsd:anyURI .

C1901A00006:238 a legcons:Item,
        skos:Concept,
        dcat:Resource ;
    rdfs:label "Item I238"@en-AU ;
    rdfs:comment "96 A  Outwards duty free shops - GraphNodeID: I238"@en-AU ;
    skos:definition "96 A  Outwards duty free shops"@en-AU ;
    skos:narrower C1901A00006:163 ;
    skos:prefLabel "Item I238"@en-AU ;
    dcat:accessURL "https://www.legislation.gov.au/C1901A00006/2024-07-01/2024-07-01/text/original/epub/OEBPS/document_1/document_1.html#_Toc172623212"^^xsd:anyURI .

C1901A00006:239 a legcons:Item,
        skos:Concept,
        dcat:Resource ;
    rdfs:label "Item I239"@en-AU ;
    rdfs:comment "96 B  Inwards duty free shops - GraphNodeID: I239"@en-AU ;
    skos:definition "96 B  Inwards duty free shops"@en-AU ;
    skos:narrower C1901A00006:163 ;
    skos:prefLabel "Item I239"@en-AU ;
    dcat:accessURL "https://www.legislation.gov.au/C1901A00006/2024-07-01/2024-07-01/text/original/epub/OEBPS/document_1/document_1.html#_Toc172623213"^^xsd:anyURI .

C1901A00006:24 a legcons:Item,
        skos:Concept,
        dcat:Resource ;
    rdfs:label "Item I24"@en-AU ;
    rdfs:comment "11  Arrangements with States and the Northern Territory - GraphNodeID: I24"@en-AU ;
    skos:definition "11  Arrangements with States and the Northern Territory"@en-AU ;
    skos:narrower C1901A00006:14 ;
    skos:prefLabel "Item I24"@en-AU ;
    dcat:accessURL "https://www.legislation.gov.au/C1901A00006/2024-07-01/2024-07-01/text/original/epub/OEBPS/document_1/document_1.html#_Toc172622998"^^xsd:anyURI .

C1901A00006:240 a legcons:Item,
        skos:Concept,
        dcat:Resource ;
    rdfs:label "Item I240"@en-AU ;
    rdfs:comment "97  Goods for public exhibition - GraphNodeID: I240"@en-AU ;
    skos:definition "97  Goods for public exhibition"@en-AU ;
    skos:narrower C1901A00006:163 ;
    skos:prefLabel "Item I240"@en-AU ;
    dcat:accessURL "https://www.legislation.gov.au/C1901A00006/2024-07-01/2024-07-01/text/original/epub/OEBPS/document_1/document_1.html#_Toc172623214"^^xsd:anyURI .

C1901A00006:241 a legcons:Item,
        skos:Concept,
        dcat:Resource ;
    rdfs:label "Item I241"@en-AU ;
    rdfs:comment "98  Goods blended or packaged in warehouse - GraphNodeID: I241"@en-AU ;
    skos:definition "98  Goods blended or packaged in warehouse"@en-AU ;
    skos:narrower C1901A00006:163 ;
    skos:prefLabel "Item I241"@en-AU ;
    dcat:accessURL "https://www.legislation.gov.au/C1901A00006/2024-07-01/2024-07-01/text/original/epub/OEBPS/document_1/document_1.html#_Toc172623215"^^xsd:anyURI .

C1901A00006:242 a legcons:Item,
        skos:Concept,
        dcat:Resource ;
    rdfs:label "Item I242"@en-AU ;
    rdfs:comment "99  Entry of warehoused goods - GraphNodeID: I242"@en-AU ;
    skos:definition "99  Entry of warehoused goods"@en-AU ;
    skos:narrower C1901A00006:163 ;
    skos:prefLabel "Item I242"@en-AU ;
    dcat:accessURL "https://www.legislation.gov.au/C1901A00006/2024-07-01/2024-07-01/text/original/epub/OEBPS/document_1/document_1.html#_Toc172623216"^^xsd:anyURI .

C1901A00006:243 a legcons:Item,
        skos:Concept,
        dcat:Resource ;
    rdfs:label "Item I243"@en-AU ;
    rdfs:comment "100  Entry of goods without warehousing with permission of Collector - GraphNodeID: I243"@en-AU ;
    skos:definition "100  Entry of goods without warehousing with permission of Collector"@en-AU ;
    skos:narrower C1901A00006:163 ;
    skos:prefLabel "Item I243"@en-AU ;
    dcat:accessURL "https://www.legislation.gov.au/C1901A00006/2024-07-01/2024-07-01/text/original/epub/OEBPS/document_1/document_1.html#_Toc172623217"^^xsd:anyURI .

C1901A00006:244 a legcons:Item,
        skos:Concept,
        dcat:Resource ;
    rdfs:label "Item I244"@en-AU ;
    rdfs:comment "101  Delivery of warehousing authority - GraphNodeID: I244"@en-AU ;
    skos:definition "101  Delivery of warehousing authority"@en-AU ;
    skos:narrower C1901A00006:163 ;
    skos:prefLabel "Item I244"@en-AU ;
    dcat:accessURL "https://www.legislation.gov.au/C1901A00006/2024-07-01/2024-07-01/text/original/epub/OEBPS/document_1/document_1.html#_Toc172623218"^^xsd:anyURI .

C1901A00006:245 a legcons:Item,
        skos:Concept,
        dcat:Resource ;
    rdfs:label "Item I245"@en-AU ;
    rdfs:comment "102  Holder of licence to inform Collector of certain matters - GraphNodeID: I245"@en-AU ;
    skos:definition "102  Holder of licence to inform Collector of certain matters"@en-AU ;
    skos:narrower C1901A00006:163 ;
    skos:prefLabel "Item I245"@en-AU ;
    dcat:accessURL "https://www.legislation.gov.au/C1901A00006/2024-07-01/2024-07-01/text/original/epub/OEBPS/document_1/document_1.html#_Toc172623219"^^xsd:anyURI .

C1901A00006:246 a legcons:Item,
        skos:Concept,
        dcat:Resource ;
    rdfs:label "Item I246"@en-AU ;
    rdfs:comment "102 A  Notices to Department by holder of warehouse licence - GraphNodeID: I246"@en-AU ;
    skos:definition "102 A  Notices to Department by holder of warehouse licence"@en-AU ;
    skos:narrower C1901A00006:163 ;
    skos:prefLabel "Item I246"@en-AU ;
    dcat:accessURL "https://www.legislation.gov.au/C1901A00006/2024-07-01/2024-07-01/text/original/epub/OEBPS/document_1/document_1.html#_Toc172623220"^^xsd:anyURI .

C1901A00006:247 a legcons:Item,
        skos:Concept,
        dcat:Resource ;
    rdfs:label "Item I247"@en-AU ;
    rdfs:comment "102 AB  Disclosure of excise equivalent warehouse licence information - GraphNodeID: I247"@en-AU ;
    skos:definition "102 AB  Disclosure of excise equivalent warehouse licence information"@en-AU ;
    skos:narrower C1901A00006:163 ;
    skos:prefLabel "Item I247"@en-AU ;
    dcat:accessURL "https://www.legislation.gov.au/C1901A00006/2024-07-01/2024-07-01/text/original/epub/OEBPS/document_1/document_1.html#_Toc172623221"^^xsd:anyURI .

C1901A00006:249 a legcons:Division,
        skos:Concept,
        dcat:Resource ;
    rdfs:label "Division D249"@en-AU ;
    rdfs:comment "Division 1 Preliminary - GraphNodeID: D249"@en-AU ;
    skos:definition "Division 1 Preliminary"@en-AU ;
    skos:narrower C1901A00006:248 ;
    skos:prefLabel "Division D249"@en-AU ;
    dcat:accessURL "https://www.legislation.gov.au/C1901A00006/2024-07-01/2024-07-01/text/original/epub/OEBPS/document_1/document_1.html#_Toc172623223"^^xsd:anyURI .

C1901A00006:25 a legcons:Item,
        skos:Concept,
        dcat:Resource ;
    rdfs:label "Item I25"@en-AU ;
    rdfs:comment "13  Customs seal - GraphNodeID: I25"@en-AU ;
    skos:definition "13  Customs seal"@en-AU ;
    skos:narrower C1901A00006:14 ;
    skos:prefLabel "Item I25"@en-AU ;
    dcat:accessURL "https://www.legislation.gov.au/C1901A00006/2024-07-01/2024-07-01/text/original/epub/OEBPS/document_1/document_1.html#_Toc172622999"^^xsd:anyURI .

C1901A00006:250 a legcons:Item,
        skos:Concept,
        dcat:Resource ;
    rdfs:label "Item I250"@en-AU ;
    rdfs:comment "102 B  Definitions - GraphNodeID: I250"@en-AU ;
    skos:definition "102 B  Definitions"@en-AU ;
    skos:narrower C1901A00006:163 ;
    skos:prefLabel "Item I250"@en-AU ;
    dcat:accessURL "https://www.legislation.gov.au/C1901A00006/2024-07-01/2024-07-01/text/original/epub/OEBPS/document_1/document_1.html#_Toc172623224"^^xsd:anyURI .

C1901A00006:251 a legcons:Item,
        skos:Concept,
        dcat:Resource ;
    rdfs:label "Item I251"@en-AU ;
    rdfs:comment "102 BA  Meaning of fit and proper person - GraphNodeID: I251"@en-AU ;
    skos:definition "102 BA  Meaning of fit and proper person"@en-AU ;
    skos:narrower C1901A00006:163 ;
    skos:prefLabel "Item I251"@en-AU ;
    dcat:accessURL "https://www.legislation.gov.au/C1901A00006/2024-07-01/2024-07-01/text/original/epub/OEBPS/document_1/document_1.html#_Toc172623225"^^xsd:anyURI .

C1901A00006:252 a legcons:Division,
        skos:Concept,
        dcat:Resource ;
    rdfs:label "Division D252"@en-AU ;
    rdfs:comment "Division 2 Obligations of cargo terminal operators - GraphNodeID: D252"@en-AU ;
    skos:definition "Division 2 Obligations of cargo terminal operators"@en-AU ;
    skos:narrower C1901A00006:248 ;
    skos:prefLabel "Division D252"@en-AU ;
    dcat:accessURL "https://www.legislation.gov.au/C1901A00006/2024-07-01/2024-07-01/text/original/epub/OEBPS/document_1/document_1.html#_Toc172623226"^^xsd:anyURI .

C1901A00006:253 a legcons:Item,
        skos:Concept,
        dcat:Resource ;
    rdfs:label "Item I253"@en-AU ;
    rdfs:comment "102 C  Notifying Department of cargo terminal - GraphNodeID: I253"@en-AU ;
    skos:definition "102 C  Notifying Department of cargo terminal"@en-AU ;
    skos:narrower C1901A00006:163 ;
    skos:prefLabel "Item I253"@en-AU ;
    dcat:accessURL "https://www.legislation.gov.au/C1901A00006/2024-07-01/2024-07-01/text/original/epub/OEBPS/document_1/document_1.html#_Toc172623227"^^xsd:anyURI .

C1901A00006:254 a legcons:Item,
        skos:Concept,
        dcat:Resource ;
    rdfs:label "Item I254"@en-AU ;
    rdfs:comment "102 CA  Physical security of cargo terminal and goods - GraphNodeID: I254"@en-AU ;
    skos:definition "102 CA  Physical security of cargo terminal and goods"@en-AU ;
    skos:narrower C1901A00006:163 ;
    skos:prefLabel "Item I254"@en-AU ;
    dcat:accessURL "https://www.legislation.gov.au/C1901A00006/2024-07-01/2024-07-01/text/original/epub/OEBPS/document_1/document_1.html#_Toc172623228"^^xsd:anyURI .

C1901A00006:255 a legcons:Item,
        skos:Concept,
        dcat:Resource ;
    rdfs:label "Item I255"@en-AU ;
    rdfs:comment "102 CB  Movement of signs at or near cargo terminal - GraphNodeID: I255"@en-AU ;
    skos:definition "102 CB  Movement of signs at or near cargo terminal"@en-AU ;
    skos:narrower C1901A00006:163 ;
    skos:prefLabel "Item I255"@en-AU ;
    dcat:accessURL "https://www.legislation.gov.au/C1901A00006/2024-07-01/2024-07-01/text/original/epub/OEBPS/document_1/document_1.html#_Toc172623229"^^xsd:anyURI .

C1901A00006:256 a legcons:Item,
        skos:Concept,
        dcat:Resource ;
    rdfs:label "Item I256"@en-AU ;
    rdfs:comment "102 CC  Notification requirements relating to goods - GraphNodeID: I256"@en-AU ;
    skos:definition "102 CC  Notification requirements relating to goods"@en-AU ;
    skos:narrower C1901A00006:163 ;
    skos:prefLabel "Item I256"@en-AU ;
    dcat:accessURL "https://www.legislation.gov.au/C1901A00006/2024-07-01/2024-07-01/text/original/epub/OEBPS/document_1/document_1.html#_Toc172623230"^^xsd:anyURI .

C1901A00006:257 a legcons:Item,
        skos:Concept,
        dcat:Resource ;
    rdfs:label "Item I257"@en-AU ;
    rdfs:comment "102 CD  Unclaimed goods - GraphNodeID: I257"@en-AU ;
    skos:definition "102 CD  Unclaimed goods"@en-AU ;
    skos:narrower C1901A00006:163 ;
    skos:prefLabel "Item I257"@en-AU ;
    dcat:accessURL "https://www.legislation.gov.au/C1901A00006/2024-07-01/2024-07-01/text/original/epub/OEBPS/document_1/document_1.html#_Toc172623231"^^xsd:anyURI .

C1901A00006:258 a legcons:Item,
        skos:Concept,
        dcat:Resource ;
    rdfs:label "Item I258"@en-AU ;
    rdfs:comment "102 CE  Record keeping requirements - GraphNodeID: I258"@en-AU ;
    skos:definition "102 CE  Record keeping requirements"@en-AU ;
    skos:narrower C1901A00006:163 ;
    skos:prefLabel "Item I258"@en-AU ;
    dcat:accessURL "https://www.legislation.gov.au/C1901A00006/2024-07-01/2024-07-01/text/original/epub/OEBPS/document_1/document_1.html#_Toc172623232"^^xsd:anyURI .

C1901A00006:259 a legcons:Item,
        skos:Concept,
        dcat:Resource ;
    rdfs:label "Item I259"@en-AU ;
    rdfs:comment "102 CF  Fit and proper person - GraphNodeID: I259"@en-AU ;
    skos:definition "102 CF  Fit and proper person"@en-AU ;
    skos:narrower C1901A00006:163 ;
    skos:prefLabel "Item I259"@en-AU ;
    dcat:accessURL "https://www.legislation.gov.au/C1901A00006/2024-07-01/2024-07-01/text/original/epub/OEBPS/document_1/document_1.html#_Toc172623233"^^xsd:anyURI .

C1901A00006:26 a legcons:Item,
        skos:Concept,
        dcat:Resource ;
    rdfs:label "Item I26"@en-AU ;
    rdfs:comment "14  Flag - GraphNodeID: I26"@en-AU ;
    skos:definition "14  Flag"@en-AU ;
    skos:narrower C1901A00006:14 ;
    skos:prefLabel "Item I26"@en-AU ;
    dcat:accessURL "https://www.legislation.gov.au/C1901A00006/2024-07-01/2024-07-01/text/original/epub/OEBPS/document_1/document_1.html#_Toc172623000"^^xsd:anyURI .

C1901A00006:260 a legcons:Item,
        skos:Concept,
        dcat:Resource ;
    rdfs:label "Item I260"@en-AU ;
    rdfs:comment "102 CG  Adequate training of staff - GraphNodeID: I260"@en-AU ;
    skos:definition "102 CG  Adequate training of staff"@en-AU ;
    skos:narrower C1901A00006:163 ;
    skos:prefLabel "Item I260"@en-AU ;
    dcat:accessURL "https://www.legislation.gov.au/C1901A00006/2024-07-01/2024-07-01/text/original/epub/OEBPS/document_1/document_1.html#_Toc172623234"^^xsd:anyURI .

C1901A00006:261 a legcons:Item,
        skos:Concept,
        dcat:Resource ;
    rdfs:label "Item I261"@en-AU ;
    rdfs:comment "102 CH  Complying with directions - GraphNodeID: I261"@en-AU ;
    skos:definition "102 CH  Complying with directions"@en-AU ;
    skos:narrower C1901A00006:163 ;
    skos:prefLabel "Item I261"@en-AU ;
    dcat:accessURL "https://www.legislation.gov.au/C1901A00006/2024-07-01/2024-07-01/text/original/epub/OEBPS/document_1/document_1.html#_Toc172623235"^^xsd:anyURI .

C1901A00006:262 a legcons:Item,
        skos:Concept,
        dcat:Resource ;
    rdfs:label "Item I262"@en-AU ;
    rdfs:comment "102 CI  Responsibility to provide facilities and assistance - GraphNodeID: I262"@en-AU ;
    skos:definition "102 CI  Responsibility to provide facilities and assistance"@en-AU ;
    skos:narrower C1901A00006:163 ;
    skos:prefLabel "Item I262"@en-AU ;
    dcat:accessURL "https://www.legislation.gov.au/C1901A00006/2024-07-01/2024-07-01/text/original/epub/OEBPS/document_1/document_1.html#_Toc172623236"^^xsd:anyURI .

C1901A00006:263 a legcons:Item,
        skos:Concept,
        dcat:Resource ;
    rdfs:label "Item I263"@en-AU ;
    rdfs:comment "102 CJ  Comptroller General of Customs may impose additional obligations - GraphNodeID: I263"@en-AU ;
    skos:definition "102 CJ  Comptroller General of Customs may impose additional obligations"@en-AU ;
    skos:narrower C1901A00006:163 ;
    skos:prefLabel "Item I263"@en-AU ;
    dcat:accessURL "https://www.legislation.gov.au/C1901A00006/2024-07-01/2024-07-01/text/original/epub/OEBPS/document_1/document_1.html#_Toc172623237"^^xsd:anyURI .

C1901A00006:264 a legcons:Item,
        skos:Concept,
        dcat:Resource ;
    rdfs:label "Item I264"@en-AU ;
    rdfs:comment "102 CK  Offencefailure to comply with obligations or requirements - GraphNodeID: I264"@en-AU ;
    skos:definition "102 CK  Offencefailure to comply with obligations or requirements"@en-AU ;
    skos:narrower C1901A00006:163 ;
    skos:prefLabel "Item I264"@en-AU ;
    dcat:accessURL "https://www.legislation.gov.au/C1901A00006/2024-07-01/2024-07-01/text/original/epub/OEBPS/document_1/document_1.html#_Toc172623238"^^xsd:anyURI .

C1901A00006:265 a legcons:Division,
        skos:Concept,
        dcat:Resource ;
    rdfs:label "Division D265"@en-AU ;
    rdfs:comment "Division 3 Obligations of cargo handlers - GraphNodeID: D265"@en-AU ;
    skos:definition "Division 3 Obligations of cargo handlers"@en-AU ;
    skos:narrower C1901A00006:248 ;
    skos:prefLabel "Division D265"@en-AU ;
    dcat:accessURL "https://www.legislation.gov.au/C1901A00006/2024-07-01/2024-07-01/text/original/epub/OEBPS/document_1/document_1.html#_Toc172623239"^^xsd:anyURI .

C1901A00006:266 a legcons:Item,
        skos:Concept,
        dcat:Resource ;
    rdfs:label "Item I266"@en-AU ;
    rdfs:comment "102 D  Certain provisions of Division 2 apply - GraphNodeID: I266"@en-AU ;
    skos:definition "102 D  Certain provisions of Division 2 apply"@en-AU ;
    skos:narrower C1901A00006:163 ;
    skos:prefLabel "Item I266"@en-AU ;
    dcat:accessURL "https://www.legislation.gov.au/C1901A00006/2024-07-01/2024-07-01/text/original/epub/OEBPS/document_1/document_1.html#_Toc172623240"^^xsd:anyURI .

C1901A00006:267 a legcons:Item,
        skos:Concept,
        dcat:Resource ;
    rdfs:label "Item I267"@en-AU ;
    rdfs:comment "102 DA  Unpacking of goods in containers at cargo terminal - GraphNodeID: I267"@en-AU ;
    skos:definition "102 DA  Unpacking of goods in containers at cargo terminal"@en-AU ;
    skos:narrower C1901A00006:163 ;
    skos:prefLabel "Item I267"@en-AU ;
    dcat:accessURL "https://www.legislation.gov.au/C1901A00006/2024-07-01/2024-07-01/text/original/epub/OEBPS/document_1/document_1.html#_Toc172623241"^^xsd:anyURI .

C1901A00006:268 a legcons:Item,
        skos:Concept,
        dcat:Resource ;
    rdfs:label "Item I268"@en-AU ;
    rdfs:comment "102 DB  Facilitating transhipment or export of goods - GraphNodeID: I268"@en-AU ;
    skos:definition "102 DB  Facilitating transhipment or export of goods"@en-AU ;
    skos:narrower C1901A00006:163 ;
    skos:prefLabel "Item I268"@en-AU ;
    dcat:accessURL "https://www.legislation.gov.au/C1901A00006/2024-07-01/2024-07-01/text/original/epub/OEBPS/document_1/document_1.html#_Toc172623242"^^xsd:anyURI .

C1901A00006:269 a legcons:Item,
        skos:Concept,
        dcat:Resource ;
    rdfs:label "Item I269"@en-AU ;
    rdfs:comment "102 DC  Using establishment identification when communicating with Department - GraphNodeID: I269"@en-AU ;
    skos:definition "102 DC  Using establishment identification when communicating with Department"@en-AU ;
    skos:narrower C1901A00006:163 ;
    skos:prefLabel "Item I269"@en-AU ;
    dcat:accessURL "https://www.legislation.gov.au/C1901A00006/2024-07-01/2024-07-01/text/original/epub/OEBPS/document_1/document_1.html#_Toc172623243"^^xsd:anyURI .

C1901A00006:27 a legcons:Item,
        skos:Concept,
        dcat:Resource ;
    rdfs:label "Item I27"@en-AU ;
    rdfs:comment "15  Appointment of ports etc - GraphNodeID: I27"@en-AU ;
    skos:definition "15  Appointment of ports etc"@en-AU ;
    skos:narrower C1901A00006:14 ;
    skos:prefLabel "Item I27"@en-AU ;
    dcat:accessURL "https://www.legislation.gov.au/C1901A00006/2024-07-01/2024-07-01/text/original/epub/OEBPS/document_1/document_1.html#_Toc172623001"^^xsd:anyURI .

C1901A00006:270 a legcons:Item,
        skos:Concept,
        dcat:Resource ;
    rdfs:label "Item I270"@en-AU ;
    rdfs:comment "102 DD  Comptroller General of Customs may impose additional obligations - GraphNodeID: I270"@en-AU ;
    skos:definition "102 DD  Comptroller General of Customs may impose additional obligations"@en-AU ;
    skos:narrower C1901A00006:163 ;
    skos:prefLabel "Item I270"@en-AU ;
    dcat:accessURL "https://www.legislation.gov.au/C1901A00006/2024-07-01/2024-07-01/text/original/epub/OEBPS/document_1/document_1.html#_Toc172623244"^^xsd:anyURI .

C1901A00006:271 a legcons:Item,
        skos:Concept,
        dcat:Resource ;
    rdfs:label "Item I271"@en-AU ;
    rdfs:comment "102 DE  Offencefailure to comply with obligations or requirements - GraphNodeID: I271"@en-AU ;
    skos:definition "102 DE  Offencefailure to comply with obligations or requirements"@en-AU ;
    skos:narrower C1901A00006:163 ;
    skos:prefLabel "Item I271"@en-AU ;
    dcat:accessURL "https://www.legislation.gov.au/C1901A00006/2024-07-01/2024-07-01/text/original/epub/OEBPS/document_1/document_1.html#_Toc172623245"^^xsd:anyURI .

C1901A00006:272 a legcons:Division,
        skos:Concept,
        dcat:Resource ;
    rdfs:label "Division D272"@en-AU ;
    rdfs:comment "Division 4 Powers of authorised officers - GraphNodeID: D272"@en-AU ;
    skos:definition "Division 4 Powers of authorised officers"@en-AU ;
    skos:narrower C1901A00006:248 ;
    skos:prefLabel "Division D272"@en-AU ;
    dcat:accessURL "https://www.legislation.gov.au/C1901A00006/2024-07-01/2024-07-01/text/original/epub/OEBPS/document_1/document_1.html#_Toc172623246"^^xsd:anyURI .

C1901A00006:273 a legcons:Item,
        skos:Concept,
        dcat:Resource ;
    rdfs:label "Item I273"@en-AU ;
    rdfs:comment "102 E  General powers - GraphNodeID: I273"@en-AU ;
    skos:definition "102 E  General powers"@en-AU ;
    skos:narrower C1901A00006:163 ;
    skos:prefLabel "Item I273"@en-AU ;
    dcat:accessURL "https://www.legislation.gov.au/C1901A00006/2024-07-01/2024-07-01/text/original/epub/OEBPS/document_1/document_1.html#_Toc172623247"^^xsd:anyURI .

C1901A00006:274 a legcons:Item,
        skos:Concept,
        dcat:Resource ;
    rdfs:label "Item I274"@en-AU ;
    rdfs:comment "102 EA  Power to make requests - GraphNodeID: I274"@en-AU ;
    skos:definition "102 EA  Power to make requests"@en-AU ;
    skos:narrower C1901A00006:163 ;
    skos:prefLabel "Item I274"@en-AU ;
    dcat:accessURL "https://www.legislation.gov.au/C1901A00006/2024-07-01/2024-07-01/text/original/epub/OEBPS/document_1/document_1.html#_Toc172623248"^^xsd:anyURI .

C1901A00006:275 a legcons:Item,
        skos:Concept,
        dcat:Resource ;
    rdfs:label "Item I275"@en-AU ;
    rdfs:comment "102 EB  Power to give directions - GraphNodeID: I275"@en-AU ;
    skos:definition "102 EB  Power to give directions"@en-AU ;
    skos:narrower C1901A00006:163 ;
    skos:prefLabel "Item I275"@en-AU ;
    dcat:accessURL "https://www.legislation.gov.au/C1901A00006/2024-07-01/2024-07-01/text/original/epub/OEBPS/document_1/document_1.html#_Toc172623249"^^xsd:anyURI .

C1901A00006:276 a legcons:Division,
        skos:Concept,
        dcat:Resource ;
    rdfs:label "Division D276"@en-AU ;
    rdfs:comment "Division 5 Directions to cargo terminal operators or cargo handlers - GraphNodeID: D276"@en-AU ;
    skos:definition "Division 5 Directions to cargo terminal operators or cargo handlers"@en-AU ;
    skos:narrower C1901A00006:248 ;
    skos:prefLabel "Division D276"@en-AU ;
    dcat:accessURL "https://www.legislation.gov.au/C1901A00006/2024-07-01/2024-07-01/text/original/epub/OEBPS/document_1/document_1.html#_Toc172623250"^^xsd:anyURI .

C1901A00006:277 a legcons:Item,
        skos:Concept,
        dcat:Resource ;
    rdfs:label "Item I277"@en-AU ;
    rdfs:comment "102 F  Directions to cargo terminal operators or cargo handlers etc - GraphNodeID: I277"@en-AU ;
    skos:definition "102 F  Directions to cargo terminal operators or cargo handlers etc"@en-AU ;
    skos:narrower C1901A00006:163 ;
    skos:prefLabel "Item I277"@en-AU ;
    dcat:accessURL "https://www.legislation.gov.au/C1901A00006/2024-07-01/2024-07-01/text/original/epub/OEBPS/document_1/document_1.html#_Toc172623251"^^xsd:anyURI .

C1901A00006:278 a legcons:Item,
        skos:Concept,
        dcat:Resource ;
    rdfs:label "Item I278"@en-AU ;
    rdfs:comment "102 FA  Offencefailure to comply with direction - GraphNodeID: I278"@en-AU ;
    skos:definition "102 FA  Offencefailure to comply with direction"@en-AU ;
    skos:narrower C1901A00006:163 ;
    skos:prefLabel "Item I278"@en-AU ;
    dcat:accessURL "https://www.legislation.gov.au/C1901A00006/2024-07-01/2024-07-01/text/original/epub/OEBPS/document_1/document_1.html#_Toc172623252"^^xsd:anyURI .

C1901A00006:279 a legcons:Part,
        skos:Concept,
        dcat:Resource ;
    rdfs:label "Part P279"@en-AU ;
    rdfs:comment "Part VASpecial provisions relating to beverages - GraphNodeID: P279"@en-AU ;
    skos:definition "Part VASpecial provisions relating to beverages"@en-AU ;
    skos:narrower C1901A00006:1 ;
    skos:prefLabel "Part P279"@en-AU ;
    dcat:accessURL "https://www.legislation.gov.au/C1901A00006/2024-07-01/2024-07-01/text/original/epub/OEBPS/document_1/document_1.html#_Toc172623253"^^xsd:anyURI .

C1901A00006:28 a legcons:Item,
        skos:Concept,
        dcat:Resource ;
    rdfs:label "Item I28"@en-AU ;
    rdfs:comment "19  Accommodation on wharfs and at airports - GraphNodeID: I28"@en-AU ;
    skos:definition "19  Accommodation on wharfs and at airports"@en-AU ;
    skos:narrower C1901A00006:14 ;
    skos:prefLabel "Item I28"@en-AU ;
    dcat:accessURL "https://www.legislation.gov.au/C1901A00006/2024-07-01/2024-07-01/text/original/epub/OEBPS/document_1/document_1.html#_Toc172623002"^^xsd:anyURI .

C1901A00006:280 a legcons:Item,
        skos:Concept,
        dcat:Resource ;
    rdfs:label "Item I280"@en-AU ;
    rdfs:comment "103  Interpretation - GraphNodeID: I280"@en-AU ;
    skos:definition "103  Interpretation"@en-AU ;
    skos:narrower C1901A00006:163 ;
    skos:prefLabel "Item I280"@en-AU ;
    dcat:accessURL "https://www.legislation.gov.au/C1901A00006/2024-07-01/2024-07-01/text/original/epub/OEBPS/document_1/document_1.html#_Toc172623254"^^xsd:anyURI .

C1901A00006:281 a legcons:Item,
        skos:Concept,
        dcat:Resource ;
    rdfs:label "Item I281"@en-AU ;
    rdfs:comment "104  Customable beverage imported in bulk must be entered for warehousing - GraphNodeID: I281"@en-AU ;
    skos:definition "104  Customable beverage imported in bulk must be entered for warehousing"@en-AU ;
    skos:narrower C1901A00006:163 ;
    skos:prefLabel "Item I281"@en-AU ;
    dcat:accessURL "https://www.legislation.gov.au/C1901A00006/2024-07-01/2024-07-01/text/original/epub/OEBPS/document_1/document_1.html#_Toc172623255"^^xsd:anyURI .

C1901A00006:282 a legcons:Item,
        skos:Concept,
        dcat:Resource ;
    rdfs:label "Item I282"@en-AU ;
    rdfs:comment "105  Certain customable beverage not to be entered for home consumption in bulk containers without approval of Comptroller General of Customs - GraphNodeID: I282"@en-AU ;
    skos:definition "105  Certain customable beverage not to be entered for home consumption in bulk containers without approval of Comptroller General of Customs"@en-AU ;
    skos:narrower C1901A00006:163 ;
    skos:prefLabel "Item I282"@en-AU ;
    dcat:accessURL "https://www.legislation.gov.au/C1901A00006/2024-07-01/2024-07-01/text/original/epub/OEBPS/document_1/document_1.html#_Toc172623256"^^xsd:anyURI .

C1901A00006:283 a legcons:Item,
        skos:Concept,
        dcat:Resource ;
    rdfs:label "Item I283"@en-AU ;
    rdfs:comment "105 A  Delivery from customs control of brandy whisky or rum - GraphNodeID: I283"@en-AU ;
    skos:definition "105 A  Delivery from customs control of brandy whisky or rum"@en-AU ;
    skos:narrower C1901A00006:163 ;
    skos:prefLabel "Item I283"@en-AU ;
    dcat:accessURL "https://www.legislation.gov.au/C1901A00006/2024-07-01/2024-07-01/text/original/epub/OEBPS/document_1/document_1.html#_Toc172623257"^^xsd:anyURI .

C1901A00006:284 a legcons:Part,
        skos:Concept,
        dcat:Resource ;
    rdfs:label "Part P284"@en-AU ;
    rdfs:comment "Part VAASpecial provisions relating to excise equivalent goods - GraphNodeID: P284"@en-AU ;
    skos:definition "Part VAASpecial provisions relating to excise equivalent goods"@en-AU ;
    skos:narrower C1901A00006:1 ;
    skos:prefLabel "Part P284"@en-AU ;
    dcat:accessURL "https://www.legislation.gov.au/C1901A00006/2024-07-01/2024-07-01/text/original/epub/OEBPS/document_1/document_1.html#_Toc172623258"^^xsd:anyURI .

C1901A00006:285 a legcons:Item,
        skos:Concept,
        dcat:Resource ;
    rdfs:label "Item I285"@en-AU ;
    rdfs:comment "105 B  Extinguishment of duty on excise equivalent goods - GraphNodeID: I285"@en-AU ;
    skos:definition "105 B  Extinguishment of duty on excise equivalent goods"@en-AU ;
    skos:narrower C1901A00006:163 ;
    skos:prefLabel "Item I285"@en-AU ;
    dcat:accessURL "https://www.legislation.gov.au/C1901A00006/2024-07-01/2024-07-01/text/original/epub/OEBPS/document_1/document_1.html#_Toc172623259"^^xsd:anyURI .

C1901A00006:286 a legcons:Item,
        skos:Concept,
        dcat:Resource ;
    rdfs:label "Item I286"@en-AU ;
    rdfs:comment "105 C  Returns - GraphNodeID: I286"@en-AU ;
    skos:definition "105 C  Returns"@en-AU ;
    skos:narrower C1901A00006:163 ;
    skos:prefLabel "Item I286"@en-AU ;
    dcat:accessURL "https://www.legislation.gov.au/C1901A00006/2024-07-01/2024-07-01/text/original/epub/OEBPS/document_1/document_1.html#_Toc172623260"^^xsd:anyURI .

C1901A00006:287 a legcons:Item,
        skos:Concept,
        dcat:Resource ;
    rdfs:label "Item I287"@en-AU ;
    rdfs:comment "105 D  GST matters - GraphNodeID: I287"@en-AU ;
    skos:definition "105 D  GST matters"@en-AU ;
    skos:narrower C1901A00006:163 ;
    skos:prefLabel "Item I287"@en-AU ;
    dcat:accessURL "https://www.legislation.gov.au/C1901A00006/2024-07-01/2024-07-01/text/original/epub/OEBPS/document_1/document_1.html#_Toc172623261"^^xsd:anyURI .

C1901A00006:288 a legcons:Item,
        skos:Concept,
        dcat:Resource ;
    rdfs:label "Item I288"@en-AU ;
    rdfs:comment "105 E  Use of excise equivalent goods in the manufacture of excisable goods to occur at a dual licensed place - GraphNodeID: I288"@en-AU ;
    skos:definition "105 E  Use of excise equivalent goods in the manufacture of excisable goods to occur at a dual licensed place"@en-AU ;
    skos:narrower C1901A00006:163 ;
    skos:prefLabel "Item I288"@en-AU ;
    dcat:accessURL "https://www.legislation.gov.au/C1901A00006/2024-07-01/2024-07-01/text/original/epub/OEBPS/document_1/document_1.html#_Toc172623262"^^xsd:anyURI .

C1901A00006:29 a legcons:Item,
        skos:Concept,
        dcat:Resource ;
    rdfs:label "Item I29"@en-AU ;
    rdfs:comment "20  Waterfront area control - GraphNodeID: I29"@en-AU ;
    skos:definition "20  Waterfront area control"@en-AU ;
    skos:narrower C1901A00006:14 ;
    skos:prefLabel "Item I29"@en-AU ;
    dcat:accessURL "https://www.legislation.gov.au/C1901A00006/2024-07-01/2024-07-01/text/original/epub/OEBPS/document_1/document_1.html#_Toc172623003"^^xsd:anyURI .

C1901A00006:292 a legcons:Item,
        skos:Concept,
        dcat:Resource ;
    rdfs:label "Item I292"@en-AU ;
    rdfs:comment "106 A  Ships and aircraft to which this Subdivision applies - GraphNodeID: I292"@en-AU ;
    skos:definition "106 A  Ships and aircraft to which this Subdivision applies"@en-AU ;
    skos:narrower C1901A00006:291 ;
    skos:prefLabel "Item I292"@en-AU ;
    dcat:accessURL "https://www.legislation.gov.au/C1901A00006/2024-07-01/2024-07-01/text/original/epub/OEBPS/document_1/document_1.html#_Toc172623266"^^xsd:anyURI .

C1901A00006:293 a legcons:Item,
        skos:Concept,
        dcat:Resource ;
    rdfs:label "Item I293"@en-AU ;
    rdfs:comment "106 B  Report 48 hours before ship or aircraft is due to depart - GraphNodeID: I293"@en-AU ;
    skos:definition "106 B  Report 48 hours before ship or aircraft is due to depart"@en-AU ;
    skos:narrower C1901A00006:291 ;
    skos:prefLabel "Item I293"@en-AU ;
    dcat:accessURL "https://www.legislation.gov.au/C1901A00006/2024-07-01/2024-07-01/text/original/epub/OEBPS/document_1/document_1.html#_Toc172623267"^^xsd:anyURI .

C1901A00006:294 a legcons:Item,
        skos:Concept,
        dcat:Resource ;
    rdfs:label "Item I294"@en-AU ;
    rdfs:comment "106 C  Report 4 hours before ship or aircraft is due to depart - GraphNodeID: I294"@en-AU ;
    skos:definition "106 C  Report 4 hours before ship or aircraft is due to depart"@en-AU ;
    skos:narrower C1901A00006:291 ;
    skos:prefLabel "Item I294"@en-AU ;
    dcat:accessURL "https://www.legislation.gov.au/C1901A00006/2024-07-01/2024-07-01/text/original/epub/OEBPS/document_1/document_1.html#_Toc172623268"^^xsd:anyURI .

C1901A00006:295 a legcons:Item,
        skos:Concept,
        dcat:Resource ;
    rdfs:label "Item I295"@en-AU ;
    rdfs:comment "106 D  Report just before ship or aircraft departs - GraphNodeID: I295"@en-AU ;
    skos:definition "106 D  Report just before ship or aircraft departs"@en-AU ;
    skos:narrower C1901A00006:291 ;
    skos:prefLabel "Item I295"@en-AU ;
    dcat:accessURL "https://www.legislation.gov.au/C1901A00006/2024-07-01/2024-07-01/text/original/epub/OEBPS/document_1/document_1.html#_Toc172623269"^^xsd:anyURI .

C1901A00006:297 a legcons:Item,
        skos:Concept,
        dcat:Resource ;
    rdfs:label "Item I297"@en-AU ;
    rdfs:comment "106 E  Ships and aircraft to which this Subdivision applies - GraphNodeID: I297"@en-AU ;
    skos:definition "106 E  Ships and aircraft to which this Subdivision applies"@en-AU ;
    skos:narrower C1901A00006:296 ;
    skos:prefLabel "Item I297"@en-AU ;
    dcat:accessURL "https://www.legislation.gov.au/C1901A00006/2024-07-01/2024-07-01/text/original/epub/OEBPS/document_1/document_1.html#_Toc172623271"^^xsd:anyURI .

C1901A00006:298 a legcons:Item,
        skos:Concept,
        dcat:Resource ;
    rdfs:label "Item I298"@en-AU ;
    rdfs:comment "106 F  Reports on matters in approved statement - GraphNodeID: I298"@en-AU ;
    skos:definition "106 F  Reports on matters in approved statement"@en-AU ;
    skos:narrower C1901A00006:296 ;
    skos:prefLabel "Item I298"@en-AU ;
    dcat:accessURL "https://www.legislation.gov.au/C1901A00006/2024-07-01/2024-07-01/text/original/epub/OEBPS/document_1/document_1.html#_Toc172623272"^^xsd:anyURI .

C1901A00006:3 a legcons:Item,
        skos:Concept,
        dcat:Resource ;
    rdfs:label "Item I3"@en-AU ;
    rdfs:comment "1  Short title - GraphNodeID: I3"@en-AU ;
    skos:definition "1  Short title"@en-AU ;
    skos:narrower C1901A00006:2 ;
    skos:prefLabel "Item I3"@en-AU ;
    dcat:accessURL "https://www.legislation.gov.au/C1901A00006/2024-07-01/2024-07-01/text/original/epub/OEBPS/document_1/document_1.html#_Toc172622977"^^xsd:anyURI .

C1901A00006:30 a legcons:Item,
        skos:Concept,
        dcat:Resource ;
    rdfs:label "Item I30"@en-AU ;
    rdfs:comment "25  Persons before whom declarations may be made - GraphNodeID: I30"@en-AU ;
    skos:definition "25  Persons before whom declarations may be made"@en-AU ;
    skos:narrower C1901A00006:14 ;
    skos:prefLabel "Item I30"@en-AU ;
    dcat:accessURL "https://www.legislation.gov.au/C1901A00006/2024-07-01/2024-07-01/text/original/epub/OEBPS/document_1/document_1.html#_Toc172623004"^^xsd:anyURI .

C1901A00006:300 a legcons:Item,
        skos:Concept,
        dcat:Resource ;
    rdfs:label "Item I300"@en-AU ;
    rdfs:comment "106 G  Reports to be made electronically - GraphNodeID: I300"@en-AU ;
    skos:definition "106 G  Reports to be made electronically"@en-AU ;
    skos:narrower C1901A00006:299 ;
    skos:prefLabel "Item I300"@en-AU ;
    dcat:accessURL "https://www.legislation.gov.au/C1901A00006/2024-07-01/2024-07-01/text/original/epub/OEBPS/document_1/document_1.html#_Toc172623274"^^xsd:anyURI .

C1901A00006:301 a legcons:Item,
        skos:Concept,
        dcat:Resource ;
    rdfs:label "Item I301"@en-AU ;
    rdfs:comment "106 H  Reports to be made by document if approved electronic system or other approved format or method unavailable - GraphNodeID: I301"@en-AU ;
    skos:definition "106 H  Reports to be made by document if approved electronic system or other approved format or method unavailable"@en-AU ;
    skos:narrower C1901A00006:299 ;
    skos:prefLabel "Item I301"@en-AU ;
    dcat:accessURL "https://www.legislation.gov.au/C1901A00006/2024-07-01/2024-07-01/text/original/epub/OEBPS/document_1/document_1.html#_Toc172623275"^^xsd:anyURI .

C1901A00006:302 a legcons:Item,
        skos:Concept,
        dcat:Resource ;
    rdfs:label "Item I302"@en-AU ;
    rdfs:comment "106 I  Comptroller General of Customs may approve different statements or forms - GraphNodeID: I302"@en-AU ;
    skos:definition "106 I  Comptroller General of Customs may approve different statements or forms"@en-AU ;
    skos:narrower C1901A00006:299 ;
    skos:prefLabel "Item I302"@en-AU ;
    dcat:accessURL "https://www.legislation.gov.au/C1901A00006/2024-07-01/2024-07-01/text/original/epub/OEBPS/document_1/document_1.html#_Toc172623276"^^xsd:anyURI .

C1901A00006:303 a legcons:Division,
        skos:Concept,
        dcat:Resource ;
    rdfs:label "Division D303"@en-AU ;
    rdfs:comment "Division 2 Questions about departing persons - GraphNodeID: D303"@en-AU ;
    skos:definition "Division 2 Questions about departing persons"@en-AU ;
    skos:narrower C1901A00006:289 ;
    skos:prefLabel "Division D303"@en-AU ;
    dcat:accessURL "https://www.legislation.gov.au/C1901A00006/2024-07-01/2024-07-01/text/original/epub/OEBPS/document_1/document_1.html#_Toc172623277"^^xsd:anyURI .

C1901A00006:304 a legcons:Item,
        skos:Concept,
        dcat:Resource ;
    rdfs:label "Item I304"@en-AU ;
    rdfs:comment "106 J  Officers may question operators about departing persons - GraphNodeID: I304"@en-AU ;
    skos:definition "106 J  Officers may question operators about departing persons"@en-AU ;
    skos:narrower C1901A00006:299 ;
    skos:prefLabel "Item I304"@en-AU ;
    dcat:accessURL "https://www.legislation.gov.au/C1901A00006/2024-07-01/2024-07-01/text/original/epub/OEBPS/document_1/document_1.html#_Toc172623278"^^xsd:anyURI .

C1901A00006:306 a legcons:Division,
        skos:Concept,
        dcat:Resource ;
    rdfs:label "Division D306"@en-AU ;
    rdfs:comment "Division 1 AAAPreliminary - GraphNodeID: D306"@en-AU ;
    skos:definition "Division 1 AAAPreliminary"@en-AU ;
    skos:narrower C1901A00006:305 ;
    skos:prefLabel "Division D306"@en-AU ;
    dcat:accessURL "https://www.legislation.gov.au/C1901A00006/2024-07-01/2024-07-01/text/original/epub/OEBPS/document_1/document_1.html#_Toc172623280"^^xsd:anyURI .

C1901A00006:307 a legcons:Item,
        skos:Concept,
        dcat:Resource ;
    rdfs:label "Item I307"@en-AU ;
    rdfs:comment "107  Obligations under this Part may be satisfied in accordance with a trusted trader agreement - GraphNodeID: I307"@en-AU ;
    skos:definition "107  Obligations under this Part may be satisfied in accordance with a trusted trader agreement"@en-AU ;
    skos:narrower C1901A00006:299 ;
    skos:prefLabel "Item I307"@en-AU ;
    dcat:accessURL "https://www.legislation.gov.au/C1901A00006/2024-07-01/2024-07-01/text/original/epub/OEBPS/document_1/document_1.html#_Toc172623281"^^xsd:anyURI .

C1901A00006:308 a legcons:Division,
        skos:Concept,
        dcat:Resource ;
    rdfs:label "Division D308"@en-AU ;
    rdfs:comment "Division 1 Prohibited exports - GraphNodeID: D308"@en-AU ;
    skos:definition "Division 1 Prohibited exports"@en-AU ;
    skos:narrower C1901A00006:305 ;
    skos:prefLabel "Division D308"@en-AU ;
    dcat:accessURL "https://www.legislation.gov.au/C1901A00006/2024-07-01/2024-07-01/text/original/epub/OEBPS/document_1/document_1.html#_Toc172623282"^^xsd:anyURI .

C1901A00006:309 a legcons:Item,
        skos:Concept,
        dcat:Resource ;
    rdfs:label "Item I309"@en-AU ;
    rdfs:comment "112  Prohibited exports - GraphNodeID: I309"@en-AU ;
    skos:definition "112  Prohibited exports"@en-AU ;
    skos:narrower C1901A00006:299 ;
    skos:prefLabel "Item I309"@en-AU ;
    dcat:accessURL "https://www.legislation.gov.au/C1901A00006/2024-07-01/2024-07-01/text/original/epub/OEBPS/document_1/document_1.html#_Toc172623283"^^xsd:anyURI .

C1901A00006:31 a legcons:Item,
        skos:Concept,
        dcat:Resource ;
    rdfs:label "Item I31"@en-AU ;
    rdfs:comment "26  Declaration by youths - GraphNodeID: I31"@en-AU ;
    skos:definition "26  Declaration by youths"@en-AU ;
    skos:narrower C1901A00006:14 ;
    skos:prefLabel "Item I31"@en-AU ;
    dcat:accessURL "https://www.legislation.gov.au/C1901A00006/2024-07-01/2024-07-01/text/original/epub/OEBPS/document_1/document_1.html#_Toc172623005"^^xsd:anyURI .

C1901A00006:310 a legcons:Item,
        skos:Concept,
        dcat:Resource ;
    rdfs:label "Item I310"@en-AU ;
    rdfs:comment "112 A  Certain controlled substances taken to be prohibited exports - GraphNodeID: I310"@en-AU ;
    skos:definition "112 A  Certain controlled substances taken to be prohibited exports"@en-AU ;
    skos:narrower C1901A00006:299 ;
    skos:prefLabel "Item I310"@en-AU ;
    dcat:accessURL "https://www.legislation.gov.au/C1901A00006/2024-07-01/2024-07-01/text/original/epub/OEBPS/document_1/document_1.html#_Toc172623284"^^xsd:anyURI .

C1901A00006:311 a legcons:Item,
        skos:Concept,
        dcat:Resource ;
    rdfs:label "Item I311"@en-AU ;
    rdfs:comment "112 B  Invalidation of licence permission etc for false or misleading information - GraphNodeID: I311"@en-AU ;
    skos:definition "112 B  Invalidation of licence permission etc for false or misleading information"@en-AU ;
    skos:narrower C1901A00006:299 ;
    skos:prefLabel "Item I311"@en-AU ;
    dcat:accessURL "https://www.legislation.gov.au/C1901A00006/2024-07-01/2024-07-01/text/original/epub/OEBPS/document_1/document_1.html#_Toc172623285"^^xsd:anyURI .

C1901A00006:312 a legcons:Division,
        skos:Concept,
        dcat:Resource ;
    rdfs:label "Division D312"@en-AU ;
    rdfs:comment "Division 1 AAExport of goods for a military end use - GraphNodeID: D312"@en-AU ;
    skos:definition "Division 1 AAExport of goods for a military end use"@en-AU ;
    skos:narrower C1901A00006:305 ;
    skos:prefLabel "Division D312"@en-AU ;
    dcat:accessURL "https://www.legislation.gov.au/C1901A00006/2024-07-01/2024-07-01/text/original/epub/OEBPS/document_1/document_1.html#_Toc172623286"^^xsd:anyURI .

C1901A00006:313 a legcons:Item,
        skos:Concept,
        dcat:Resource ;
    rdfs:label "Item I313"@en-AU ;
    rdfs:comment "112 BA  Notice prohibiting export - GraphNodeID: I313"@en-AU ;
    skos:definition "112 BA  Notice prohibiting export"@en-AU ;
    skos:narrower C1901A00006:299 ;
    skos:prefLabel "Item I313"@en-AU ;
    dcat:accessURL "https://www.legislation.gov.au/C1901A00006/2024-07-01/2024-07-01/text/original/epub/OEBPS/document_1/document_1.html#_Toc172623287"^^xsd:anyURI .

C1901A00006:314 a legcons:Item,
        skos:Concept,
        dcat:Resource ;
    rdfs:label "Item I314"@en-AU ;
    rdfs:comment "112 BB  How notices are to be given - GraphNodeID: I314"@en-AU ;
    skos:definition "112 BB  How notices are to be given"@en-AU ;
    skos:narrower C1901A00006:299 ;
    skos:prefLabel "Item I314"@en-AU ;
    dcat:accessURL "https://www.legislation.gov.au/C1901A00006/2024-07-01/2024-07-01/text/original/epub/OEBPS/document_1/document_1.html#_Toc172623288"^^xsd:anyURI .

C1901A00006:315 a legcons:Item,
        skos:Concept,
        dcat:Resource ;
    rdfs:label "Item I315"@en-AU ;
    rdfs:comment "112 BC  Statement to Parliament - GraphNodeID: I315"@en-AU ;
    skos:definition "112 BC  Statement to Parliament"@en-AU ;
    skos:narrower C1901A00006:299 ;
    skos:prefLabel "Item I315"@en-AU ;
    dcat:accessURL "https://www.legislation.gov.au/C1901A00006/2024-07-01/2024-07-01/text/original/epub/OEBPS/document_1/document_1.html#_Toc172623289"^^xsd:anyURI .

C1901A00006:316 a legcons:Division,
        skos:Concept,
        dcat:Resource ;
    rdfs:label "Division D316"@en-AU ;
    rdfs:comment "Division 1 ADirections in relation to goods for export etc that are subject to customs control - GraphNodeID: D316"@en-AU ;
    skos:definition "Division 1 ADirections in relation to goods for export etc that are subject to customs control"@en-AU ;
    skos:narrower C1901A00006:305 ;
    skos:prefLabel "Division D316"@en-AU ;
    dcat:accessURL "https://www.legislation.gov.au/C1901A00006/2024-07-01/2024-07-01/text/original/epub/OEBPS/document_1/document_1.html#_Toc172623290"^^xsd:anyURI .

C1901A00006:317 a legcons:Item,
        skos:Concept,
        dcat:Resource ;
    rdfs:label "Item I317"@en-AU ;
    rdfs:comment "112 C  Collector may give directions in relation to goods for export etc that are subject to customs control - GraphNodeID: I317"@en-AU ;
    skos:definition "112 C  Collector may give directions in relation to goods for export etc that are subject to customs control"@en-AU ;
    skos:narrower C1901A00006:299 ;
    skos:prefLabel "Item I317"@en-AU ;
    dcat:accessURL "https://www.legislation.gov.au/C1901A00006/2024-07-01/2024-07-01/text/original/epub/OEBPS/document_1/document_1.html#_Toc172623291"^^xsd:anyURI .

C1901A00006:318 a legcons:Item,
        skos:Concept,
        dcat:Resource ;
    rdfs:label "Item I318"@en-AU ;
    rdfs:comment "112 D  Compliance with a direction given under section 112 C - GraphNodeID: I318"@en-AU ;
    skos:definition "112 D  Compliance with a direction given under section 112 C"@en-AU ;
    skos:narrower C1901A00006:299 ;
    skos:prefLabel "Item I318"@en-AU ;
    dcat:accessURL "https://www.legislation.gov.au/C1901A00006/2024-07-01/2024-07-01/text/original/epub/OEBPS/document_1/document_1.html#_Toc172623292"^^xsd:anyURI .

C1901A00006:32 a legcons:Item,
        skos:Concept,
        dcat:Resource ;
    rdfs:label "Item I32"@en-AU ;
    rdfs:comment "28  Working days and hours etc - GraphNodeID: I32"@en-AU ;
    skos:definition "28  Working days and hours etc"@en-AU ;
    skos:narrower C1901A00006:14 ;
    skos:prefLabel "Item I32"@en-AU ;
    dcat:accessURL "https://www.legislation.gov.au/C1901A00006/2024-07-01/2024-07-01/text/original/epub/OEBPS/document_1/document_1.html#_Toc172623006"^^xsd:anyURI .

C1901A00006:321 a legcons:Item,
        skos:Concept,
        dcat:Resource ;
    rdfs:label "Item I321"@en-AU ;
    rdfs:comment "113  Entry of goods for export - GraphNodeID: I321"@en-AU ;
    skos:definition "113  Entry of goods for export"@en-AU ;
    skos:narrower C1901A00006:320 ;
    skos:prefLabel "Item I321"@en-AU ;
    dcat:accessURL "https://www.legislation.gov.au/C1901A00006/2024-07-01/2024-07-01/text/original/epub/OEBPS/document_1/document_1.html#_Toc172623295"^^xsd:anyURI .

C1901A00006:322 a legcons:Item,
        skos:Concept,
        dcat:Resource ;
    rdfs:label "Item I322"@en-AU ;
    rdfs:comment "113 AA  How an entry of goods for export is made - GraphNodeID: I322"@en-AU ;
    skos:definition "113 AA  How an entry of goods for export is made"@en-AU ;
    skos:narrower C1901A00006:320 ;
    skos:prefLabel "Item I322"@en-AU ;
    dcat:accessURL "https://www.legislation.gov.au/C1901A00006/2024-07-01/2024-07-01/text/original/epub/OEBPS/document_1/document_1.html#_Toc172623296"^^xsd:anyURI .

C1901A00006:324 a legcons:Item,
        skos:Concept,
        dcat:Resource ;
    rdfs:label "Item I324"@en-AU ;
    rdfs:comment "114  Making an export declaration - GraphNodeID: I324"@en-AU ;
    skos:definition "114  Making an export declaration"@en-AU ;
    skos:narrower C1901A00006:323 ;
    skos:prefLabel "Item I324"@en-AU ;
    dcat:accessURL "https://www.legislation.gov.au/C1901A00006/2024-07-01/2024-07-01/text/original/epub/OEBPS/document_1/document_1.html#_Toc172623298"^^xsd:anyURI .

C1901A00006:325 a legcons:Item,
        skos:Concept,
        dcat:Resource ;
    rdfs:label "Item I325"@en-AU ;
    rdfs:comment "114 A  An officer may seek additional information - GraphNodeID: I325"@en-AU ;
    skos:definition "114 A  An officer may seek additional information"@en-AU ;
    skos:narrower C1901A00006:323 ;
    skos:prefLabel "Item I325"@en-AU ;
    dcat:accessURL "https://www.legislation.gov.au/C1901A00006/2024-07-01/2024-07-01/text/original/epub/OEBPS/document_1/document_1.html#_Toc172623299"^^xsd:anyURI .

C1901A00006:326 a legcons:Item,
        skos:Concept,
        dcat:Resource ;
    rdfs:label "Item I326"@en-AU ;
    rdfs:comment "114 B  Confirming exporters - GraphNodeID: I326"@en-AU ;
    skos:definition "114 B  Confirming exporters"@en-AU ;
    skos:narrower C1901A00006:323 ;
    skos:prefLabel "Item I326"@en-AU ;
    dcat:accessURL "https://www.legislation.gov.au/C1901A00006/2024-07-01/2024-07-01/text/original/epub/OEBPS/document_1/document_1.html#_Toc172623300"^^xsd:anyURI .

C1901A00006:328 a legcons:Item,
        skos:Concept,
        dcat:Resource ;
    rdfs:label "Item I328"@en-AU ;
    rdfs:comment "114 C  Authority to deal with goods entered for export - GraphNodeID: I328"@en-AU ;
    skos:definition "114 C  Authority to deal with goods entered for export"@en-AU ;
    skos:narrower C1901A00006:327 ;
    skos:prefLabel "Item I328"@en-AU ;
    dcat:accessURL "https://www.legislation.gov.au/C1901A00006/2024-07-01/2024-07-01/text/original/epub/OEBPS/document_1/document_1.html#_Toc172623302"^^xsd:anyURI .

C1901A00006:329 a legcons:Item,
        skos:Concept,
        dcat:Resource ;
    rdfs:label "Item I329"@en-AU ;
    rdfs:comment "114 CA  Suspension of an authority to deal with goods entered for export in order to verify particulars of the goods - GraphNodeID: I329"@en-AU ;
    skos:definition "114 CA  Suspension of an authority to deal with goods entered for export in order to verify particulars of the goods"@en-AU ;
    skos:narrower C1901A00006:327 ;
    skos:prefLabel "Item I329"@en-AU ;
    dcat:accessURL "https://www.legislation.gov.au/C1901A00006/2024-07-01/2024-07-01/text/original/epub/OEBPS/document_1/document_1.html#_Toc172623303"^^xsd:anyURI .

C1901A00006:330 a legcons:Item,
        skos:Concept,
        dcat:Resource ;
    rdfs:label "Item I330"@en-AU ;
    rdfs:comment "114 CB  Revocation of the suspension of an authority to deal - GraphNodeID: I330"@en-AU ;
    skos:definition "114 CB  Revocation of the suspension of an authority to deal"@en-AU ;
    skos:narrower C1901A00006:327 ;
    skos:prefLabel "Item I330"@en-AU ;
    dcat:accessURL "https://www.legislation.gov.au/C1901A00006/2024-07-01/2024-07-01/text/original/epub/OEBPS/document_1/document_1.html#_Toc172623304"^^xsd:anyURI .

C1901A00006:331 a legcons:Item,
        skos:Concept,
        dcat:Resource ;
    rdfs:label "Item I331"@en-AU ;
    rdfs:comment "114 CC  An officer may seek additional information if an authority to deal has been suspended - GraphNodeID: I331"@en-AU ;
    skos:definition "114 CC  An officer may seek additional information if an authority to deal has been suspended"@en-AU ;
    skos:narrower C1901A00006:327 ;
    skos:prefLabel "Item I331"@en-AU ;
    dcat:accessURL "https://www.legislation.gov.au/C1901A00006/2024-07-01/2024-07-01/text/original/epub/OEBPS/document_1/document_1.html#_Toc172623305"^^xsd:anyURI .

C1901A00006:332 a legcons:Item,
        skos:Concept,
        dcat:Resource ;
    rdfs:label "Item I332"@en-AU ;
    rdfs:comment "114 D  Goods to be dealt with in accordance with export entry - GraphNodeID: I332"@en-AU ;
    skos:definition "114 D  Goods to be dealt with in accordance with export entry"@en-AU ;
    skos:narrower C1901A00006:327 ;
    skos:prefLabel "Item I332"@en-AU ;
    dcat:accessURL "https://www.legislation.gov.au/C1901A00006/2024-07-01/2024-07-01/text/original/epub/OEBPS/document_1/document_1.html#_Toc172623306"^^xsd:anyURI .

C1901A00006:333 a legcons:Item,
        skos:Concept,
        dcat:Resource ;
    rdfs:label "Item I333"@en-AU ;
    rdfs:comment "114 E  Sending goods to a wharf or airport for export - GraphNodeID: I333"@en-AU ;
    skos:definition "114 E  Sending goods to a wharf or airport for export"@en-AU ;
    skos:narrower C1901A00006:327 ;
    skos:prefLabel "Item I333"@en-AU ;
    dcat:accessURL "https://www.legislation.gov.au/C1901A00006/2024-07-01/2024-07-01/text/original/epub/OEBPS/document_1/document_1.html#_Toc172623307"^^xsd:anyURI .

C1901A00006:334 a legcons:Item,
        skos:Concept,
        dcat:Resource ;
    rdfs:label "Item I334"@en-AU ;
    rdfs:comment "114 F  Notices to Department by person who receives goods at a wharf or airport for export - GraphNodeID: I334"@en-AU ;
    skos:definition "114 F  Notices to Department by person who receives goods at a wharf or airport for export"@en-AU ;
    skos:narrower C1901A00006:327 ;
    skos:prefLabel "Item I334"@en-AU ;
    dcat:accessURL "https://www.legislation.gov.au/C1901A00006/2024-07-01/2024-07-01/text/original/epub/OEBPS/document_1/document_1.html#_Toc172623308"^^xsd:anyURI .

C1901A00006:335 a legcons:Item,
        skos:Concept,
        dcat:Resource ;
    rdfs:label "Item I335"@en-AU ;
    rdfs:comment "115  Goods not to be taken on board without authority to deal - GraphNodeID: I335"@en-AU ;
    skos:definition "115  Goods not to be taken on board without authority to deal"@en-AU ;
    skos:narrower C1901A00006:327 ;
    skos:prefLabel "Item I335"@en-AU ;
    dcat:accessURL "https://www.legislation.gov.au/C1901A00006/2024-07-01/2024-07-01/text/original/epub/OEBPS/document_1/document_1.html#_Toc172623309"^^xsd:anyURI .

C1901A00006:336 a legcons:Item,
        skos:Concept,
        dcat:Resource ;
    rdfs:label "Item I336"@en-AU ;
    rdfs:comment "116  What happens when goods entered for export by an export declaration are not dealt with in accordance with the export entry - GraphNodeID: I336"@en-AU ;
    skos:definition "116  What happens when goods entered for export by an export declaration are not dealt with in accordance with the export entry"@en-AU ;
    skos:narrower C1901A00006:327 ;
    skos:prefLabel "Item I336"@en-AU ;
    dcat:accessURL "https://www.legislation.gov.au/C1901A00006/2024-07-01/2024-07-01/text/original/epub/OEBPS/document_1/document_1.html#_Toc172623310"^^xsd:anyURI .

C1901A00006:337 a legcons:Item,
        skos:Concept,
        dcat:Resource ;
    rdfs:label "Item I337"@en-AU ;
    rdfs:comment "117  Security - GraphNodeID: I337"@en-AU ;
    skos:definition "117  Security"@en-AU ;
    skos:narrower C1901A00006:327 ;
    skos:prefLabel "Item I337"@en-AU ;
    dcat:accessURL "https://www.legislation.gov.au/C1901A00006/2024-07-01/2024-07-01/text/original/epub/OEBPS/document_1/document_1.html#_Toc172623311"^^xsd:anyURI .

C1901A00006:338 a legcons:Item,
        skos:Concept,
        dcat:Resource ;
    rdfs:label "Item I338"@en-AU ;
    rdfs:comment "117 AA  Consolidation of certain goods for export can only occur at a prescribed place - GraphNodeID: I338"@en-AU ;
    skos:definition "117 AA  Consolidation of certain goods for export can only occur at a prescribed place"@en-AU ;
    skos:narrower C1901A00006:327 ;
    skos:prefLabel "Item I338"@en-AU ;
    dcat:accessURL "https://www.legislation.gov.au/C1901A00006/2024-07-01/2024-07-01/text/original/epub/OEBPS/document_1/document_1.html#_Toc172623312"^^xsd:anyURI .

C1901A00006:339 a legcons:Item,
        skos:Concept,
        dcat:Resource ;
    rdfs:label "Item I339"@en-AU ;
    rdfs:comment "117 A  Submanifests to be communicated to Department - GraphNodeID: I339"@en-AU ;
    skos:definition "117 A  Submanifests to be communicated to Department"@en-AU ;
    skos:narrower C1901A00006:327 ;
    skos:prefLabel "Item I339"@en-AU ;
    dcat:accessURL "https://www.legislation.gov.au/C1901A00006/2024-07-01/2024-07-01/text/original/epub/OEBPS/document_1/document_1.html#_Toc172623313"^^xsd:anyURI .

C1901A00006:34 a legcons:Item,
        skos:Concept,
        dcat:Resource ;
    rdfs:label "Item I34"@en-AU ;
    rdfs:comment "30  Customs control of goods - GraphNodeID: I34"@en-AU ;
    skos:definition "30  Customs control of goods"@en-AU ;
    skos:narrower C1901A00006:33 ;
    skos:prefLabel "Item I34"@en-AU ;
    dcat:accessURL "https://www.legislation.gov.au/C1901A00006/2024-07-01/2024-07-01/text/original/epub/OEBPS/document_1/document_1.html#_Toc172623008"^^xsd:anyURI .

C1901A00006:340 a legcons:Item,
        skos:Concept,
        dcat:Resource ;
    rdfs:label "Item I340"@en-AU ;
    rdfs:comment "118  Certificate of Clearance - GraphNodeID: I340"@en-AU ;
    skos:definition "118  Certificate of Clearance"@en-AU ;
    skos:narrower C1901A00006:327 ;
    skos:prefLabel "Item I340"@en-AU ;
    dcat:accessURL "https://www.legislation.gov.au/C1901A00006/2024-07-01/2024-07-01/text/original/epub/OEBPS/document_1/document_1.html#_Toc172623314"^^xsd:anyURI .

C1901A00006:341 a legcons:Item,
        skos:Concept,
        dcat:Resource ;
    rdfs:label "Item I341"@en-AU ;
    rdfs:comment "118 A  Requirements for granting a Certificate of Clearance in respect of certain ships or aircraft - GraphNodeID: I341"@en-AU ;
    skos:definition "118 A  Requirements for granting a Certificate of Clearance in respect of certain ships or aircraft"@en-AU ;
    skos:narrower C1901A00006:327 ;
    skos:prefLabel "Item I341"@en-AU ;
    dcat:accessURL "https://www.legislation.gov.au/C1901A00006/2024-07-01/2024-07-01/text/original/epub/OEBPS/document_1/document_1.html#_Toc172623315"^^xsd:anyURI .

C1901A00006:342 a legcons:Item,
        skos:Concept,
        dcat:Resource ;
    rdfs:label "Item I342"@en-AU ;
    rdfs:comment "119  Communication of outward manifest to Department - GraphNodeID: I342"@en-AU ;
    skos:definition "119  Communication of outward manifest to Department"@en-AU ;
    skos:narrower C1901A00006:327 ;
    skos:prefLabel "Item I342"@en-AU ;
    dcat:accessURL "https://www.legislation.gov.au/C1901A00006/2024-07-01/2024-07-01/text/original/epub/OEBPS/document_1/document_1.html#_Toc172623316"^^xsd:anyURI .

C1901A00006:343 a legcons:Item,
        skos:Concept,
        dcat:Resource ;
    rdfs:label "Item I343"@en-AU ;
    rdfs:comment "119 AA  Application for permission to move alter or interfere with goods for export - GraphNodeID: I343"@en-AU ;
    skos:definition "119 AA  Application for permission to move alter or interfere with goods for export"@en-AU ;
    skos:narrower C1901A00006:327 ;
    skos:prefLabel "Item I343"@en-AU ;
    dcat:accessURL "https://www.legislation.gov.au/C1901A00006/2024-07-01/2024-07-01/text/original/epub/OEBPS/document_1/document_1.html#_Toc172623317"^^xsd:anyURI .

C1901A00006:344 a legcons:Item,
        skos:Concept,
        dcat:Resource ;
    rdfs:label "Item I344"@en-AU ;
    rdfs:comment "119 AB  Application for permission to move alter or interfere with goods that are no longer for export - GraphNodeID: I344"@en-AU ;
    skos:definition "119 AB  Application for permission to move alter or interfere with goods that are no longer for export"@en-AU ;
    skos:narrower C1901A00006:327 ;
    skos:prefLabel "Item I344"@en-AU ;
    dcat:accessURL "https://www.legislation.gov.au/C1901A00006/2024-07-01/2024-07-01/text/original/epub/OEBPS/document_1/document_1.html#_Toc172623318"^^xsd:anyURI .

C1901A00006:345 a legcons:Item,
        skos:Concept,
        dcat:Resource ;
    rdfs:label "Item I345"@en-AU ;
    rdfs:comment "119 AC  Dealing with an application for a permission to move etc goods that are no longer for export - GraphNodeID: I345"@en-AU ;
    skos:definition "119 AC  Dealing with an application for a permission to move etc goods that are no longer for export"@en-AU ;
    skos:narrower C1901A00006:327 ;
    skos:prefLabel "Item I345"@en-AU ;
    dcat:accessURL "https://www.legislation.gov.au/C1901A00006/2024-07-01/2024-07-01/text/original/epub/OEBPS/document_1/document_1.html#_Toc172623319"^^xsd:anyURI .

C1901A00006:346 a legcons:Item,
        skos:Concept,
        dcat:Resource ;
    rdfs:label "Item I346"@en-AU ;
    rdfs:comment "119 A  Withdrawal of entries submanifests and manifests - GraphNodeID: I346"@en-AU ;
    skos:definition "119 A  Withdrawal of entries submanifests and manifests"@en-AU ;
    skos:narrower C1901A00006:327 ;
    skos:prefLabel "Item I346"@en-AU ;
    dcat:accessURL "https://www.legislation.gov.au/C1901A00006/2024-07-01/2024-07-01/text/original/epub/OEBPS/document_1/document_1.html#_Toc172623320"^^xsd:anyURI .

C1901A00006:347 a legcons:Item,
        skos:Concept,
        dcat:Resource ;
    rdfs:label "Item I347"@en-AU ;
    rdfs:comment "119 B  Effect of withdrawal - GraphNodeID: I347"@en-AU ;
    skos:definition "119 B  Effect of withdrawal"@en-AU ;
    skos:narrower C1901A00006:327 ;
    skos:prefLabel "Item I347"@en-AU ;
    dcat:accessURL "https://www.legislation.gov.au/C1901A00006/2024-07-01/2024-07-01/text/original/epub/OEBPS/document_1/document_1.html#_Toc172623321"^^xsd:anyURI .

C1901A00006:348 a legcons:Item,
        skos:Concept,
        dcat:Resource ;
    rdfs:label "Item I348"@en-AU ;
    rdfs:comment "119 C  Change of electronic entries and change of submanifests and manifests treated as withdrawals - GraphNodeID: I348"@en-AU ;
    skos:definition "119 C  Change of electronic entries and change of submanifests and manifests treated as withdrawals"@en-AU ;
    skos:narrower C1901A00006:327 ;
    skos:prefLabel "Item I348"@en-AU ;
    dcat:accessURL "https://www.legislation.gov.au/C1901A00006/2024-07-01/2024-07-01/text/original/epub/OEBPS/document_1/document_1.html#_Toc172623322"^^xsd:anyURI .

C1901A00006:349 a legcons:Item,
        skos:Concept,
        dcat:Resource ;
    rdfs:label "Item I349"@en-AU ;
    rdfs:comment "119 D  Notification of export entries submanifests manifests withdrawals and applications - GraphNodeID: I349"@en-AU ;
    skos:definition "119 D  Notification of export entries submanifests manifests withdrawals and applications"@en-AU ;
    skos:narrower C1901A00006:327 ;
    skos:prefLabel "Item I349"@en-AU ;
    dcat:accessURL "https://www.legislation.gov.au/C1901A00006/2024-07-01/2024-07-01/text/original/epub/OEBPS/document_1/document_1.html#_Toc172623323"^^xsd:anyURI .

C1901A00006:35 a legcons:Item,
        skos:Concept,
        dcat:Resource ;
    rdfs:label "Item I35"@en-AU ;
    rdfs:comment "30 A  Exemptions under Torres Strait Treaty - GraphNodeID: I35"@en-AU ;
    skos:definition "30 A  Exemptions under Torres Strait Treaty"@en-AU ;
    skos:narrower C1901A00006:33 ;
    skos:prefLabel "Item I35"@en-AU ;
    dcat:accessURL "https://www.legislation.gov.au/C1901A00006/2024-07-01/2024-07-01/text/original/epub/OEBPS/document_1/document_1.html#_Toc172623009"^^xsd:anyURI .

C1901A00006:350 a legcons:Item,
        skos:Concept,
        dcat:Resource ;
    rdfs:label "Item I350"@en-AU ;
    rdfs:comment "119 E  Requirements for communicating to Department electronically - GraphNodeID: I350"@en-AU ;
    skos:definition "119 E  Requirements for communicating to Department electronically"@en-AU ;
    skos:narrower C1901A00006:327 ;
    skos:prefLabel "Item I350"@en-AU ;
    dcat:accessURL "https://www.legislation.gov.au/C1901A00006/2024-07-01/2024-07-01/text/original/epub/OEBPS/document_1/document_1.html#_Toc172623324"^^xsd:anyURI .

C1901A00006:351 a legcons:Item,
        skos:Concept,
        dcat:Resource ;
    rdfs:label "Item I351"@en-AU ;
    rdfs:comment "120  Shipment of goods - GraphNodeID: I351"@en-AU ;
    skos:definition "120  Shipment of goods"@en-AU ;
    skos:narrower C1901A00006:327 ;
    skos:prefLabel "Item I351"@en-AU ;
    dcat:accessURL "https://www.legislation.gov.au/C1901A00006/2024-07-01/2024-07-01/text/original/epub/OEBPS/document_1/document_1.html#_Toc172623325"^^xsd:anyURI .

C1901A00006:352 a legcons:Item,
        skos:Concept,
        dcat:Resource ;
    rdfs:label "Item I352"@en-AU ;
    rdfs:comment "122  Time of clearance - GraphNodeID: I352"@en-AU ;
    skos:definition "122  Time of clearance"@en-AU ;
    skos:narrower C1901A00006:327 ;
    skos:prefLabel "Item I352"@en-AU ;
    dcat:accessURL "https://www.legislation.gov.au/C1901A00006/2024-07-01/2024-07-01/text/original/epub/OEBPS/document_1/document_1.html#_Toc172623326"^^xsd:anyURI .

C1901A00006:353 a legcons:Division,
        skos:Concept,
        dcat:Resource ;
    rdfs:label "Division D353"@en-AU ;
    rdfs:comment "Division 3 AExamining goods for export that are not yet subject to customs control - GraphNodeID: D353"@en-AU ;
    skos:definition "Division 3 AExamining goods for export that are not yet subject to customs control"@en-AU ;
    skos:narrower C1901A00006:305 ;
    skos:prefLabel "Division D353"@en-AU ;
    dcat:accessURL "https://www.legislation.gov.au/C1901A00006/2024-07-01/2024-07-01/text/original/epub/OEBPS/document_1/document_1.html#_Toc172623327"^^xsd:anyURI .

C1901A00006:354 a legcons:Item,
        skos:Concept,
        dcat:Resource ;
    rdfs:label "Item I354"@en-AU ;
    rdfs:comment "122 F  Object of Division - GraphNodeID: I354"@en-AU ;
    skos:definition "122 F  Object of Division"@en-AU ;
    skos:narrower C1901A00006:327 ;
    skos:prefLabel "Item I354"@en-AU ;
    dcat:accessURL "https://www.legislation.gov.au/C1901A00006/2024-07-01/2024-07-01/text/original/epub/OEBPS/document_1/document_1.html#_Toc172623328"^^xsd:anyURI .

C1901A00006:355 a legcons:Item,
        skos:Concept,
        dcat:Resource ;
    rdfs:label "Item I355"@en-AU ;
    rdfs:comment "122 G  Occupier of premises - GraphNodeID: I355"@en-AU ;
    skos:definition "122 G  Occupier of premises"@en-AU ;
    skos:narrower C1901A00006:327 ;
    skos:prefLabel "Item I355"@en-AU ;
    dcat:accessURL "https://www.legislation.gov.au/C1901A00006/2024-07-01/2024-07-01/text/original/epub/OEBPS/document_1/document_1.html#_Toc172623329"^^xsd:anyURI .

C1901A00006:356 a legcons:Item,
        skos:Concept,
        dcat:Resource ;
    rdfs:label "Item I356"@en-AU ;
    rdfs:comment "122 H  Consent required to enter premises and examine goods for export - GraphNodeID: I356"@en-AU ;
    skos:definition "122 H  Consent required to enter premises and examine goods for export"@en-AU ;
    skos:narrower C1901A00006:327 ;
    skos:prefLabel "Item I356"@en-AU ;
    dcat:accessURL "https://www.legislation.gov.au/C1901A00006/2024-07-01/2024-07-01/text/original/epub/OEBPS/document_1/document_1.html#_Toc172623330"^^xsd:anyURI .

C1901A00006:357 a legcons:Item,
        skos:Concept,
        dcat:Resource ;
    rdfs:label "Item I357"@en-AU ;
    rdfs:comment "122 J  Officer must leave premises if consent withdrawn - GraphNodeID: I357"@en-AU ;
    skos:definition "122 J  Officer must leave premises if consent withdrawn"@en-AU ;
    skos:narrower C1901A00006:327 ;
    skos:prefLabel "Item I357"@en-AU ;
    dcat:accessURL "https://www.legislation.gov.au/C1901A00006/2024-07-01/2024-07-01/text/original/epub/OEBPS/document_1/document_1.html#_Toc172623331"^^xsd:anyURI .

C1901A00006:358 a legcons:Item,
        skos:Concept,
        dcat:Resource ;
    rdfs:label "Item I358"@en-AU ;
    rdfs:comment "122 K  Power to search premises for export goods - GraphNodeID: I358"@en-AU ;
    skos:definition "122 K  Power to search premises for export goods"@en-AU ;
    skos:narrower C1901A00006:327 ;
    skos:prefLabel "Item I358"@en-AU ;
    dcat:accessURL "https://www.legislation.gov.au/C1901A00006/2024-07-01/2024-07-01/text/original/epub/OEBPS/document_1/document_1.html#_Toc172623332"^^xsd:anyURI .

C1901A00006:359 a legcons:Item,
        skos:Concept,
        dcat:Resource ;
    rdfs:label "Item I359"@en-AU ;
    rdfs:comment "122 L  Power to examine export goods - GraphNodeID: I359"@en-AU ;
    skos:definition "122 L  Power to examine export goods"@en-AU ;
    skos:narrower C1901A00006:327 ;
    skos:prefLabel "Item I359"@en-AU ;
    dcat:accessURL "https://www.legislation.gov.au/C1901A00006/2024-07-01/2024-07-01/text/original/epub/OEBPS/document_1/document_1.html#_Toc172623333"^^xsd:anyURI .

C1901A00006:36 a legcons:Item,
        skos:Concept,
        dcat:Resource ;
    rdfs:label "Item I36"@en-AU ;
    rdfs:comment "31  Goods on ships and aircraft subject to customs control - GraphNodeID: I36"@en-AU ;
    skos:definition "31  Goods on ships and aircraft subject to customs control"@en-AU ;
    skos:narrower C1901A00006:33 ;
    skos:prefLabel "Item I36"@en-AU ;
    dcat:accessURL "https://www.legislation.gov.au/C1901A00006/2024-07-01/2024-07-01/text/original/epub/OEBPS/document_1/document_1.html#_Toc172623010"^^xsd:anyURI .

C1901A00006:360 a legcons:Item,
        skos:Concept,
        dcat:Resource ;
    rdfs:label "Item I360"@en-AU ;
    rdfs:comment "122 M  Power to examine documents relating to export goods - GraphNodeID: I360"@en-AU ;
    skos:definition "122 M  Power to examine documents relating to export goods"@en-AU ;
    skos:narrower C1901A00006:327 ;
    skos:prefLabel "Item I360"@en-AU ;
    dcat:accessURL "https://www.legislation.gov.au/C1901A00006/2024-07-01/2024-07-01/text/original/epub/OEBPS/document_1/document_1.html#_Toc172623334"^^xsd:anyURI .

C1901A00006:361 a legcons:Item,
        skos:Concept,
        dcat:Resource ;
    rdfs:label "Item I361"@en-AU ;
    rdfs:comment "122 N  Power to question occupier about export goods - GraphNodeID: I361"@en-AU ;
    skos:definition "122 N  Power to question occupier about export goods"@en-AU ;
    skos:narrower C1901A00006:327 ;
    skos:prefLabel "Item I361"@en-AU ;
    dcat:accessURL "https://www.legislation.gov.au/C1901A00006/2024-07-01/2024-07-01/text/original/epub/OEBPS/document_1/document_1.html#_Toc172623335"^^xsd:anyURI .

C1901A00006:362 a legcons:Item,
        skos:Concept,
        dcat:Resource ;
    rdfs:label "Item I362"@en-AU ;
    rdfs:comment "122 P  Power to bring equipment to the premises - GraphNodeID: I362"@en-AU ;
    skos:definition "122 P  Power to bring equipment to the premises"@en-AU ;
    skos:narrower C1901A00006:327 ;
    skos:prefLabel "Item I362"@en-AU ;
    dcat:accessURL "https://www.legislation.gov.au/C1901A00006/2024-07-01/2024-07-01/text/original/epub/OEBPS/document_1/document_1.html#_Toc172623336"^^xsd:anyURI .

C1901A00006:363 a legcons:Item,
        skos:Concept,
        dcat:Resource ;
    rdfs:label "Item I363"@en-AU ;
    rdfs:comment "122 Q  Compensation - GraphNodeID: I363"@en-AU ;
    skos:definition "122 Q  Compensation"@en-AU ;
    skos:narrower C1901A00006:327 ;
    skos:prefLabel "Item I363"@en-AU ;
    dcat:accessURL "https://www.legislation.gov.au/C1901A00006/2024-07-01/2024-07-01/text/original/epub/OEBPS/document_1/document_1.html#_Toc172623337"^^xsd:anyURI .

C1901A00006:364 a legcons:Item,
        skos:Concept,
        dcat:Resource ;
    rdfs:label "Item I364"@en-AU ;
    rdfs:comment "122 R  Powers in this Division are additional to other powers - GraphNodeID: I364"@en-AU ;
    skos:definition "122 R  Powers in this Division are additional to other powers"@en-AU ;
    skos:narrower C1901A00006:327 ;
    skos:prefLabel "Item I364"@en-AU ;
    dcat:accessURL "https://www.legislation.gov.au/C1901A00006/2024-07-01/2024-07-01/text/original/epub/OEBPS/document_1/document_1.html#_Toc172623338"^^xsd:anyURI .

C1901A00006:365 a legcons:Division,
        skos:Concept,
        dcat:Resource ;
    rdfs:label "Division D365"@en-AU ;
    rdfs:comment "Division 4 Exportation procedures after Certificate of Clearance issued - GraphNodeID: D365"@en-AU ;
    skos:definition "Division 4 Exportation procedures after Certificate of Clearance issued"@en-AU ;
    skos:narrower C1901A00006:305 ;
    skos:prefLabel "Division D365"@en-AU ;
    dcat:accessURL "https://www.legislation.gov.au/C1901A00006/2024-07-01/2024-07-01/text/original/epub/OEBPS/document_1/document_1.html#_Toc172623339"^^xsd:anyURI .

C1901A00006:366 a legcons:Item,
        skos:Concept,
        dcat:Resource ;
    rdfs:label "Item I366"@en-AU ;
    rdfs:comment "123  Ship to bring to and aircraft to stop at boarding stations - GraphNodeID: I366"@en-AU ;
    skos:definition "123  Ship to bring to and aircraft to stop at boarding stations"@en-AU ;
    skos:narrower C1901A00006:327 ;
    skos:prefLabel "Item I366"@en-AU ;
    dcat:accessURL "https://www.legislation.gov.au/C1901A00006/2024-07-01/2024-07-01/text/original/epub/OEBPS/document_1/document_1.html#_Toc172623340"^^xsd:anyURI .

C1901A00006:367 a legcons:Item,
        skos:Concept,
        dcat:Resource ;
    rdfs:label "Item I367"@en-AU ;
    rdfs:comment "124  Master or pilot to account for missing goods - GraphNodeID: I367"@en-AU ;
    skos:definition "124  Master or pilot to account for missing goods"@en-AU ;
    skos:narrower C1901A00006:327 ;
    skos:prefLabel "Item I367"@en-AU ;
    dcat:accessURL "https://www.legislation.gov.au/C1901A00006/2024-07-01/2024-07-01/text/original/epub/OEBPS/document_1/document_1.html#_Toc172623341"^^xsd:anyURI .

C1901A00006:368 a legcons:Item,
        skos:Concept,
        dcat:Resource ;
    rdfs:label "Item I368"@en-AU ;
    rdfs:comment "125  Goods exported to be landed at proper destination - GraphNodeID: I368"@en-AU ;
    skos:definition "125  Goods exported to be landed at proper destination"@en-AU ;
    skos:narrower C1901A00006:327 ;
    skos:prefLabel "Item I368"@en-AU ;
    dcat:accessURL "https://www.legislation.gov.au/C1901A00006/2024-07-01/2024-07-01/text/original/epub/OEBPS/document_1/document_1.html#_Toc172623342"^^xsd:anyURI .

C1901A00006:369 a legcons:Item,
        skos:Concept,
        dcat:Resource ;
    rdfs:label "Item I369"@en-AU ;
    rdfs:comment "126  Certificate of landing - GraphNodeID: I369"@en-AU ;
    skos:definition "126  Certificate of landing"@en-AU ;
    skos:narrower C1901A00006:327 ;
    skos:prefLabel "Item I369"@en-AU ;
    dcat:accessURL "https://www.legislation.gov.au/C1901A00006/2024-07-01/2024-07-01/text/original/epub/OEBPS/document_1/document_1.html#_Toc172623343"^^xsd:anyURI .

C1901A00006:37 a legcons:Item,
        skos:Concept,
        dcat:Resource ;
    rdfs:label "Item I37"@en-AU ;
    rdfs:comment "33  Persons not to move goods subject to customs control - GraphNodeID: I37"@en-AU ;
    skos:definition "33  Persons not to move goods subject to customs control"@en-AU ;
    skos:narrower C1901A00006:33 ;
    skos:prefLabel "Item I37"@en-AU ;
    dcat:accessURL "https://www.legislation.gov.au/C1901A00006/2024-07-01/2024-07-01/text/original/epub/OEBPS/document_1/document_1.html#_Toc172623011"^^xsd:anyURI .

C1901A00006:370 a legcons:Division,
        skos:Concept,
        dcat:Resource ;
    rdfs:label "Division D370"@en-AU ;
    rdfs:comment "Division 4 AExportation of goods to Singapore - GraphNodeID: D370"@en-AU ;
    skos:definition "Division 4 AExportation of goods to Singapore"@en-AU ;
    skos:narrower C1901A00006:305 ;
    skos:prefLabel "Division D370"@en-AU ;
    dcat:accessURL "https://www.legislation.gov.au/C1901A00006/2024-07-01/2024-07-01/text/original/epub/OEBPS/document_1/document_1.html#_Toc172623344"^^xsd:anyURI .

C1901A00006:371 a legcons:Item,
        skos:Concept,
        dcat:Resource ;
    rdfs:label "Item I371"@en-AU ;
    rdfs:comment "126 AAA  Definitions - GraphNodeID: I371"@en-AU ;
    skos:definition "126 AAA  Definitions"@en-AU ;
    skos:narrower C1901A00006:327 ;
    skos:prefLabel "Item I371"@en-AU ;
    dcat:accessURL "https://www.legislation.gov.au/C1901A00006/2024-07-01/2024-07-01/text/original/epub/OEBPS/document_1/document_1.html#_Toc172623345"^^xsd:anyURI .

C1901A00006:372 a legcons:Item,
        skos:Concept,
        dcat:Resource ;
    rdfs:label "Item I372"@en-AU ;
    rdfs:comment "126 AB  Record keeping obligations - GraphNodeID: I372"@en-AU ;
    skos:definition "126 AB  Record keeping obligations"@en-AU ;
    skos:narrower C1901A00006:327 ;
    skos:prefLabel "Item I372"@en-AU ;
    dcat:accessURL "https://www.legislation.gov.au/C1901A00006/2024-07-01/2024-07-01/text/original/epub/OEBPS/document_1/document_1.html#_Toc172623346"^^xsd:anyURI .

C1901A00006:373 a legcons:Item,
        skos:Concept,
        dcat:Resource ;
    rdfs:label "Item I373"@en-AU ;
    rdfs:comment "126 AC  Power to require records - GraphNodeID: I373"@en-AU ;
    skos:definition "126 AC  Power to require records"@en-AU ;
    skos:narrower C1901A00006:327 ;
    skos:prefLabel "Item I373"@en-AU ;
    dcat:accessURL "https://www.legislation.gov.au/C1901A00006/2024-07-01/2024-07-01/text/original/epub/OEBPS/document_1/document_1.html#_Toc172623347"^^xsd:anyURI .

C1901A00006:374 a legcons:Item,
        skos:Concept,
        dcat:Resource ;
    rdfs:label "Item I374"@en-AU ;
    rdfs:comment "126 AD  Power to ask questions - GraphNodeID: I374"@en-AU ;
    skos:definition "126 AD  Power to ask questions"@en-AU ;
    skos:narrower C1901A00006:327 ;
    skos:prefLabel "Item I374"@en-AU ;
    dcat:accessURL "https://www.legislation.gov.au/C1901A00006/2024-07-01/2024-07-01/text/original/epub/OEBPS/document_1/document_1.html#_Toc172623348"^^xsd:anyURI .

C1901A00006:375 a legcons:Division,
        skos:Concept,
        dcat:Resource ;
    rdfs:label "Division D375"@en-AU ;
    rdfs:comment "Division 4 BExportation of textile or apparel goods to the US - GraphNodeID: D375"@en-AU ;
    skos:definition "Division 4 BExportation of textile or apparel goods to the US"@en-AU ;
    skos:narrower C1901A00006:305 ;
    skos:prefLabel "Division D375"@en-AU ;
    dcat:accessURL "https://www.legislation.gov.au/C1901A00006/2024-07-01/2024-07-01/text/original/epub/OEBPS/document_1/document_1.html#_Toc172623349"^^xsd:anyURI .

C1901A00006:376 a legcons:Item,
        skos:Concept,
        dcat:Resource ;
    rdfs:label "Item I376"@en-AU ;
    rdfs:comment "126 AE  Authorised officer may request records or ask questions - GraphNodeID: I376"@en-AU ;
    skos:definition "126 AE  Authorised officer may request records or ask questions"@en-AU ;
    skos:narrower C1901A00006:327 ;
    skos:prefLabel "Item I376"@en-AU ;
    dcat:accessURL "https://www.legislation.gov.au/C1901A00006/2024-07-01/2024-07-01/text/original/epub/OEBPS/document_1/document_1.html#_Toc172623350"^^xsd:anyURI .

C1901A00006:377 a legcons:Division,
        skos:Concept,
        dcat:Resource ;
    rdfs:label "Division D377"@en-AU ;
    rdfs:comment "Division 4 CExportation of goods to Thailand - GraphNodeID: D377"@en-AU ;
    skos:definition "Division 4 CExportation of goods to Thailand"@en-AU ;
    skos:narrower C1901A00006:305 ;
    skos:prefLabel "Division D377"@en-AU ;
    dcat:accessURL "https://www.legislation.gov.au/C1901A00006/2024-07-01/2024-07-01/text/original/epub/OEBPS/document_1/document_1.html#_Toc172623351"^^xsd:anyURI .

C1901A00006:378 a legcons:Item,
        skos:Concept,
        dcat:Resource ;
    rdfs:label "Item I378"@en-AU ;
    rdfs:comment "126 AF  Definitions - GraphNodeID: I378"@en-AU ;
    skos:definition "126 AF  Definitions"@en-AU ;
    skos:narrower C1901A00006:327 ;
    skos:prefLabel "Item I378"@en-AU ;
    dcat:accessURL "https://www.legislation.gov.au/C1901A00006/2024-07-01/2024-07-01/text/original/epub/OEBPS/document_1/document_1.html#_Toc172623352"^^xsd:anyURI .

C1901A00006:379 a legcons:Item,
        skos:Concept,
        dcat:Resource ;
    rdfs:label "Item I379"@en-AU ;
    rdfs:comment "126 AG  Record keeping obligations - GraphNodeID: I379"@en-AU ;
    skos:definition "126 AG  Record keeping obligations"@en-AU ;
    skos:narrower C1901A00006:327 ;
    skos:prefLabel "Item I379"@en-AU ;
    dcat:accessURL "https://www.legislation.gov.au/C1901A00006/2024-07-01/2024-07-01/text/original/epub/OEBPS/document_1/document_1.html#_Toc172623353"^^xsd:anyURI .

C1901A00006:38 a legcons:Item,
        skos:Concept,
        dcat:Resource ;
    rdfs:label "Item I38"@en-AU ;
    rdfs:comment "33 A  Resources installations subject to customs control - GraphNodeID: I38"@en-AU ;
    skos:definition "33 A  Resources installations subject to customs control"@en-AU ;
    skos:narrower C1901A00006:33 ;
    skos:prefLabel "Item I38"@en-AU ;
    dcat:accessURL "https://www.legislation.gov.au/C1901A00006/2024-07-01/2024-07-01/text/original/epub/OEBPS/document_1/document_1.html#_Toc172623012"^^xsd:anyURI .

C1901A00006:380 a legcons:Item,
        skos:Concept,
        dcat:Resource ;
    rdfs:label "Item I380"@en-AU ;
    rdfs:comment "126 AH  Power to require records - GraphNodeID: I380"@en-AU ;
    skos:definition "126 AH  Power to require records"@en-AU ;
    skos:narrower C1901A00006:327 ;
    skos:prefLabel "Item I380"@en-AU ;
    dcat:accessURL "https://www.legislation.gov.au/C1901A00006/2024-07-01/2024-07-01/text/original/epub/OEBPS/document_1/document_1.html#_Toc172623354"^^xsd:anyURI .

C1901A00006:381 a legcons:Item,
        skos:Concept,
        dcat:Resource ;
    rdfs:label "Item I381"@en-AU ;
    rdfs:comment "126 AI  Power to ask questions - GraphNodeID: I381"@en-AU ;
    skos:definition "126 AI  Power to ask questions"@en-AU ;
    skos:narrower C1901A00006:327 ;
    skos:prefLabel "Item I381"@en-AU ;
    dcat:accessURL "https://www.legislation.gov.au/C1901A00006/2024-07-01/2024-07-01/text/original/epub/OEBPS/document_1/document_1.html#_Toc172623355"^^xsd:anyURI .

C1901A00006:382 a legcons:Division,
        skos:Concept,
        dcat:Resource ;
    rdfs:label "Division D382"@en-AU ;
    rdfs:comment "Division 4 DExportation of goods to New Zealand - GraphNodeID: D382"@en-AU ;
    skos:definition "Division 4 DExportation of goods to New Zealand"@en-AU ;
    skos:narrower C1901A00006:305 ;
    skos:prefLabel "Division D382"@en-AU ;
    dcat:accessURL "https://www.legislation.gov.au/C1901A00006/2024-07-01/2024-07-01/text/original/epub/OEBPS/document_1/document_1.html#_Toc172623356"^^xsd:anyURI .

C1901A00006:383 a legcons:Item,
        skos:Concept,
        dcat:Resource ;
    rdfs:label "Item I383"@en-AU ;
    rdfs:comment "126 AJA  Definitions - GraphNodeID: I383"@en-AU ;
    skos:definition "126 AJA  Definitions"@en-AU ;
    skos:narrower C1901A00006:327 ;
    skos:prefLabel "Item I383"@en-AU ;
    dcat:accessURL "https://www.legislation.gov.au/C1901A00006/2024-07-01/2024-07-01/text/original/epub/OEBPS/document_1/document_1.html#_Toc172623357"^^xsd:anyURI .

C1901A00006:384 a legcons:Item,
        skos:Concept,
        dcat:Resource ;
    rdfs:label "Item I384"@en-AU ;
    rdfs:comment "126 AJB  Record keeping obligations - GraphNodeID: I384"@en-AU ;
    skos:definition "126 AJB  Record keeping obligations"@en-AU ;
    skos:narrower C1901A00006:327 ;
    skos:prefLabel "Item I384"@en-AU ;
    dcat:accessURL "https://www.legislation.gov.au/C1901A00006/2024-07-01/2024-07-01/text/original/epub/OEBPS/document_1/document_1.html#_Toc172623358"^^xsd:anyURI .

C1901A00006:385 a legcons:Item,
        skos:Concept,
        dcat:Resource ;
    rdfs:label "Item I385"@en-AU ;
    rdfs:comment "126 AJC  Power to require records - GraphNodeID: I385"@en-AU ;
    skos:definition "126 AJC  Power to require records"@en-AU ;
    skos:narrower C1901A00006:327 ;
    skos:prefLabel "Item I385"@en-AU ;
    dcat:accessURL "https://www.legislation.gov.au/C1901A00006/2024-07-01/2024-07-01/text/original/epub/OEBPS/document_1/document_1.html#_Toc172623359"^^xsd:anyURI .

C1901A00006:386 a legcons:Item,
        skos:Concept,
        dcat:Resource ;
    rdfs:label "Item I386"@en-AU ;
    rdfs:comment "126 AJD  Power to ask questions - GraphNodeID: I386"@en-AU ;
    skos:definition "126 AJD  Power to ask questions"@en-AU ;
    skos:narrower C1901A00006:327 ;
    skos:prefLabel "Item I386"@en-AU ;
    dcat:accessURL "https://www.legislation.gov.au/C1901A00006/2024-07-01/2024-07-01/text/original/epub/OEBPS/document_1/document_1.html#_Toc172623360"^^xsd:anyURI .

C1901A00006:387 a legcons:Division,
        skos:Concept,
        dcat:Resource ;
    rdfs:label "Division D387"@en-AU ;
    rdfs:comment "Division 4 DAExportation of goods to Peru - GraphNodeID: D387"@en-AU ;
    skos:definition "Division 4 DAExportation of goods to Peru"@en-AU ;
    skos:narrower C1901A00006:305 ;
    skos:prefLabel "Division D387"@en-AU ;
    dcat:accessURL "https://www.legislation.gov.au/C1901A00006/2024-07-01/2024-07-01/text/original/epub/OEBPS/document_1/document_1.html#_Toc172623361"^^xsd:anyURI .

C1901A00006:388 a legcons:Item,
        skos:Concept,
        dcat:Resource ;
    rdfs:label "Item I388"@en-AU ;
    rdfs:comment "126 AJE  Definitions - GraphNodeID: I388"@en-AU ;
    skos:definition "126 AJE  Definitions"@en-AU ;
    skos:narrower C1901A00006:327 ;
    skos:prefLabel "Item I388"@en-AU ;
    dcat:accessURL "https://www.legislation.gov.au/C1901A00006/2024-07-01/2024-07-01/text/original/epub/OEBPS/document_1/document_1.html#_Toc172623362"^^xsd:anyURI .

C1901A00006:389 a legcons:Item,
        skos:Concept,
        dcat:Resource ;
    rdfs:label "Item I389"@en-AU ;
    rdfs:comment "126 AJF  Record keeping obligations - GraphNodeID: I389"@en-AU ;
    skos:definition "126 AJF  Record keeping obligations"@en-AU ;
    skos:narrower C1901A00006:327 ;
    skos:prefLabel "Item I389"@en-AU ;
    dcat:accessURL "https://www.legislation.gov.au/C1901A00006/2024-07-01/2024-07-01/text/original/epub/OEBPS/document_1/document_1.html#_Toc172623363"^^xsd:anyURI .

C1901A00006:39 a legcons:Item,
        skos:Concept,
        dcat:Resource ;
    rdfs:label "Item I39"@en-AU ;
    rdfs:comment "33 B  Sea installations subject to customs control - GraphNodeID: I39"@en-AU ;
    skos:definition "33 B  Sea installations subject to customs control"@en-AU ;
    skos:narrower C1901A00006:33 ;
    skos:prefLabel "Item I39"@en-AU ;
    dcat:accessURL "https://www.legislation.gov.au/C1901A00006/2024-07-01/2024-07-01/text/original/epub/OEBPS/document_1/document_1.html#_Toc172623013"^^xsd:anyURI .

C1901A00006:390 a legcons:Item,
        skos:Concept,
        dcat:Resource ;
    rdfs:label "Item I390"@en-AU ;
    rdfs:comment "126 AJG  Power to require records - GraphNodeID: I390"@en-AU ;
    skos:definition "126 AJG  Power to require records"@en-AU ;
    skos:narrower C1901A00006:327 ;
    skos:prefLabel "Item I390"@en-AU ;
    dcat:accessURL "https://www.legislation.gov.au/C1901A00006/2024-07-01/2024-07-01/text/original/epub/OEBPS/document_1/document_1.html#_Toc172623364"^^xsd:anyURI .

C1901A00006:391 a legcons:Item,
        skos:Concept,
        dcat:Resource ;
    rdfs:label "Item I391"@en-AU ;
    rdfs:comment "126 AJH  Power to ask questions - GraphNodeID: I391"@en-AU ;
    skos:definition "126 AJH  Power to ask questions"@en-AU ;
    skos:narrower C1901A00006:327 ;
    skos:prefLabel "Item I391"@en-AU ;
    dcat:accessURL "https://www.legislation.gov.au/C1901A00006/2024-07-01/2024-07-01/text/original/epub/OEBPS/document_1/document_1.html#_Toc172623365"^^xsd:anyURI .

C1901A00006:392 a legcons:Division,
        skos:Concept,
        dcat:Resource ;
    rdfs:label "Division D392"@en-AU ;
    rdfs:comment "Division 4 EExportation of goods to Chile - GraphNodeID: D392"@en-AU ;
    skos:definition "Division 4 EExportation of goods to Chile"@en-AU ;
    skos:narrower C1901A00006:305 ;
    skos:prefLabel "Division D392"@en-AU ;
    dcat:accessURL "https://www.legislation.gov.au/C1901A00006/2024-07-01/2024-07-01/text/original/epub/OEBPS/document_1/document_1.html#_Toc172623366"^^xsd:anyURI .

C1901A00006:393 a legcons:Item,
        skos:Concept,
        dcat:Resource ;
    rdfs:label "Item I393"@en-AU ;
    rdfs:comment "126 AKA  Definitions - GraphNodeID: I393"@en-AU ;
    skos:definition "126 AKA  Definitions"@en-AU ;
    skos:narrower C1901A00006:327 ;
    skos:prefLabel "Item I393"@en-AU ;
    dcat:accessURL "https://www.legislation.gov.au/C1901A00006/2024-07-01/2024-07-01/text/original/epub/OEBPS/document_1/document_1.html#_Toc172623367"^^xsd:anyURI .

C1901A00006:394 a legcons:Item,
        skos:Concept,
        dcat:Resource ;
    rdfs:label "Item I394"@en-AU ;
    rdfs:comment "126 AKB  Record keeping obligations - GraphNodeID: I394"@en-AU ;
    skos:definition "126 AKB  Record keeping obligations"@en-AU ;
    skos:narrower C1901A00006:327 ;
    skos:prefLabel "Item I394"@en-AU ;
    dcat:accessURL "https://www.legislation.gov.au/C1901A00006/2024-07-01/2024-07-01/text/original/epub/OEBPS/document_1/document_1.html#_Toc172623368"^^xsd:anyURI .

C1901A00006:395 a legcons:Item,
        skos:Concept,
        dcat:Resource ;
    rdfs:label "Item I395"@en-AU ;
    rdfs:comment "126 AKC  Power to require records - GraphNodeID: I395"@en-AU ;
    skos:definition "126 AKC  Power to require records"@en-AU ;
    skos:narrower C1901A00006:327 ;
    skos:prefLabel "Item I395"@en-AU ;
    dcat:accessURL "https://www.legislation.gov.au/C1901A00006/2024-07-01/2024-07-01/text/original/epub/OEBPS/document_1/document_1.html#_Toc172623369"^^xsd:anyURI .

C1901A00006:396 a legcons:Item,
        skos:Concept,
        dcat:Resource ;
    rdfs:label "Item I396"@en-AU ;
    rdfs:comment "126 AKD  Power to ask questions - GraphNodeID: I396"@en-AU ;
    skos:definition "126 AKD  Power to ask questions"@en-AU ;
    skos:narrower C1901A00006:327 ;
    skos:prefLabel "Item I396"@en-AU ;
    dcat:accessURL "https://www.legislation.gov.au/C1901A00006/2024-07-01/2024-07-01/text/original/epub/OEBPS/document_1/document_1.html#_Toc172623370"^^xsd:anyURI .

C1901A00006:397 a legcons:Division,
        skos:Concept,
        dcat:Resource ;
    rdfs:label "Division D397"@en-AU ;
    rdfs:comment "Division 4 EAExportation of goods to Parties to the Pacific Agreement on Closer Economic Relations Plus - GraphNodeID: D397"@en-AU ;
    skos:definition "Division 4 EAExportation of goods to Parties to the Pacific Agreement on Closer Economic Relations Plus"@en-AU ;
    skos:narrower C1901A00006:305 ;
    skos:prefLabel "Division D397"@en-AU ;
    dcat:accessURL "https://www.legislation.gov.au/C1901A00006/2024-07-01/2024-07-01/text/original/epub/OEBPS/document_1/document_1.html#_Toc172623371"^^xsd:anyURI .

C1901A00006:398 a legcons:Item,
        skos:Concept,
        dcat:Resource ;
    rdfs:label "Item I398"@en-AU ;
    rdfs:comment "126 AKE  Definitions - GraphNodeID: I398"@en-AU ;
    skos:definition "126 AKE  Definitions"@en-AU ;
    skos:narrower C1901A00006:327 ;
    skos:prefLabel "Item I398"@en-AU ;
    dcat:accessURL "https://www.legislation.gov.au/C1901A00006/2024-07-01/2024-07-01/text/original/epub/OEBPS/document_1/document_1.html#_Toc172623372"^^xsd:anyURI .

C1901A00006:399 a legcons:Item,
        skos:Concept,
        dcat:Resource ;
    rdfs:label "Item I399"@en-AU ;
    rdfs:comment "126 AKF  Record keeping obligations - GraphNodeID: I399"@en-AU ;
    skos:definition "126 AKF  Record keeping obligations"@en-AU ;
    skos:narrower C1901A00006:327 ;
    skos:prefLabel "Item I399"@en-AU ;
    dcat:accessURL "https://www.legislation.gov.au/C1901A00006/2024-07-01/2024-07-01/text/original/epub/OEBPS/document_1/document_1.html#_Toc172623373"^^xsd:anyURI .

C1901A00006:4 a legcons:Item,
        skos:Concept,
        dcat:Resource ;
    rdfs:label "Item I4"@en-AU ;
    rdfs:comment "2  Commencement - GraphNodeID: I4"@en-AU ;
    skos:definition "2  Commencement"@en-AU ;
    skos:narrower C1901A00006:2 ;
    skos:prefLabel "Item I4"@en-AU ;
    dcat:accessURL "https://www.legislation.gov.au/C1901A00006/2024-07-01/2024-07-01/text/original/epub/OEBPS/document_1/document_1.html#_Toc172622978"^^xsd:anyURI .

C1901A00006:40 a legcons:Item,
        skos:Concept,
        dcat:Resource ;
    rdfs:label "Item I40"@en-AU ;
    rdfs:comment "33 BA  Offshore electricity installations subject to customs control - GraphNodeID: I40"@en-AU ;
    skos:definition "33 BA  Offshore electricity installations subject to customs control"@en-AU ;
    skos:narrower C1901A00006:33 ;
    skos:prefLabel "Item I40"@en-AU ;
    dcat:accessURL "https://www.legislation.gov.au/C1901A00006/2024-07-01/2024-07-01/text/original/epub/OEBPS/document_1/document_1.html#_Toc172623014"^^xsd:anyURI .

C1901A00006:400 a legcons:Item,
        skos:Concept,
        dcat:Resource ;
    rdfs:label "Item I400"@en-AU ;
    rdfs:comment "126 AKG  Power to require records - GraphNodeID: I400"@en-AU ;
    skos:definition "126 AKG  Power to require records"@en-AU ;
    skos:narrower C1901A00006:327 ;
    skos:prefLabel "Item I400"@en-AU ;
    dcat:accessURL "https://www.legislation.gov.au/C1901A00006/2024-07-01/2024-07-01/text/original/epub/OEBPS/document_1/document_1.html#_Toc172623374"^^xsd:anyURI .

C1901A00006:401 a legcons:Item,
        skos:Concept,
        dcat:Resource ;
    rdfs:label "Item I401"@en-AU ;
    rdfs:comment "126 AKH  Power to ask questions - GraphNodeID: I401"@en-AU ;
    skos:definition "126 AKH  Power to ask questions"@en-AU ;
    skos:narrower C1901A00006:327 ;
    skos:prefLabel "Item I401"@en-AU ;
    dcat:accessURL "https://www.legislation.gov.au/C1901A00006/2024-07-01/2024-07-01/text/original/epub/OEBPS/document_1/document_1.html#_Toc172623375"^^xsd:anyURI .

C1901A00006:402 a legcons:Division,
        skos:Concept,
        dcat:Resource ;
    rdfs:label "Division D402"@en-AU ;
    rdfs:comment "Division 4 EBExportation of goods to Parties to the Comprehensive and Progressive Agreement for Trans Pacific Partnership - GraphNodeID: D402"@en-AU ;
    skos:definition "Division 4 EBExportation of goods to Parties to the Comprehensive and Progressive Agreement for Trans Pacific Partnership"@en-AU ;
    skos:narrower C1901A00006:305 ;
    skos:prefLabel "Division D402"@en-AU ;
    dcat:accessURL "https://www.legislation.gov.au/C1901A00006/2024-07-01/2024-07-01/text/original/epub/OEBPS/document_1/document_1.html#_Toc172623376"^^xsd:anyURI .

C1901A00006:403 a legcons:Item,
        skos:Concept,
        dcat:Resource ;
    rdfs:label "Item I403"@en-AU ;
    rdfs:comment "126 AKI  Definitions - GraphNodeID: I403"@en-AU ;
    skos:definition "126 AKI  Definitions"@en-AU ;
    skos:narrower C1901A00006:327 ;
    skos:prefLabel "Item I403"@en-AU ;
    dcat:accessURL "https://www.legislation.gov.au/C1901A00006/2024-07-01/2024-07-01/text/original/epub/OEBPS/document_1/document_1.html#_Toc172623377"^^xsd:anyURI .

C1901A00006:404 a legcons:Item,
        skos:Concept,
        dcat:Resource ;
    rdfs:label "Item I404"@en-AU ;
    rdfs:comment "126 AKJ  Record keeping obligations - GraphNodeID: I404"@en-AU ;
    skos:definition "126 AKJ  Record keeping obligations"@en-AU ;
    skos:narrower C1901A00006:327 ;
    skos:prefLabel "Item I404"@en-AU ;
    dcat:accessURL "https://www.legislation.gov.au/C1901A00006/2024-07-01/2024-07-01/text/original/epub/OEBPS/document_1/document_1.html#_Toc172623378"^^xsd:anyURI .

C1901A00006:405 a legcons:Item,
        skos:Concept,
        dcat:Resource ;
    rdfs:label "Item I405"@en-AU ;
    rdfs:comment "126 AKK  Power to require records - GraphNodeID: I405"@en-AU ;
    skos:definition "126 AKK  Power to require records"@en-AU ;
    skos:narrower C1901A00006:327 ;
    skos:prefLabel "Item I405"@en-AU ;
    dcat:accessURL "https://www.legislation.gov.au/C1901A00006/2024-07-01/2024-07-01/text/original/epub/OEBPS/document_1/document_1.html#_Toc172623379"^^xsd:anyURI .

C1901A00006:406 a legcons:Item,
        skos:Concept,
        dcat:Resource ;
    rdfs:label "Item I406"@en-AU ;
    rdfs:comment "126 AKL  Power to ask questions - GraphNodeID: I406"@en-AU ;
    skos:definition "126 AKL  Power to ask questions"@en-AU ;
    skos:narrower C1901A00006:327 ;
    skos:prefLabel "Item I406"@en-AU ;
    dcat:accessURL "https://www.legislation.gov.au/C1901A00006/2024-07-01/2024-07-01/text/original/epub/OEBPS/document_1/document_1.html#_Toc172623380"^^xsd:anyURI .

C1901A00006:407 a legcons:Division,
        skos:Concept,
        dcat:Resource ;
    rdfs:label "Division D407"@en-AU ;
    rdfs:comment "Division 4 FExportation of goods to Malaysia - GraphNodeID: D407"@en-AU ;
    skos:definition "Division 4 FExportation of goods to Malaysia"@en-AU ;
    skos:narrower C1901A00006:305 ;
    skos:prefLabel "Division D407"@en-AU ;
    dcat:accessURL "https://www.legislation.gov.au/C1901A00006/2024-07-01/2024-07-01/text/original/epub/OEBPS/document_1/document_1.html#_Toc172623381"^^xsd:anyURI .

C1901A00006:408 a legcons:Item,
        skos:Concept,
        dcat:Resource ;
    rdfs:label "Item I408"@en-AU ;
    rdfs:comment "126 ALA  Definitions - GraphNodeID: I408"@en-AU ;
    skos:definition "126 ALA  Definitions"@en-AU ;
    skos:narrower C1901A00006:327 ;
    skos:prefLabel "Item I408"@en-AU ;
    dcat:accessURL "https://www.legislation.gov.au/C1901A00006/2024-07-01/2024-07-01/text/original/epub/OEBPS/document_1/document_1.html#_Toc172623382"^^xsd:anyURI .

C1901A00006:409 a legcons:Item,
        skos:Concept,
        dcat:Resource ;
    rdfs:label "Item I409"@en-AU ;
    rdfs:comment "126 ALB  Record keeping obligations - GraphNodeID: I409"@en-AU ;
    skos:definition "126 ALB  Record keeping obligations"@en-AU ;
    skos:narrower C1901A00006:327 ;
    skos:prefLabel "Item I409"@en-AU ;
    dcat:accessURL "https://www.legislation.gov.au/C1901A00006/2024-07-01/2024-07-01/text/original/epub/OEBPS/document_1/document_1.html#_Toc172623383"^^xsd:anyURI .

C1901A00006:41 a legcons:Item,
        skos:Concept,
        dcat:Resource ;
    rdfs:label "Item I41"@en-AU ;
    rdfs:comment "33 C  Obstructing or interfering with Commonwealth property in a Customs place - GraphNodeID: I41"@en-AU ;
    skos:definition "33 C  Obstructing or interfering with Commonwealth property in a Customs place"@en-AU ;
    skos:narrower C1901A00006:33 ;
    skos:prefLabel "Item I41"@en-AU ;
    dcat:accessURL "https://www.legislation.gov.au/C1901A00006/2024-07-01/2024-07-01/text/original/epub/OEBPS/document_1/document_1.html#_Toc172623015"^^xsd:anyURI .

C1901A00006:410 a legcons:Item,
        skos:Concept,
        dcat:Resource ;
    rdfs:label "Item I410"@en-AU ;
    rdfs:comment "126 ALC  Power to require records - GraphNodeID: I410"@en-AU ;
    skos:definition "126 ALC  Power to require records"@en-AU ;
    skos:narrower C1901A00006:327 ;
    skos:prefLabel "Item I410"@en-AU ;
    dcat:accessURL "https://www.legislation.gov.au/C1901A00006/2024-07-01/2024-07-01/text/original/epub/OEBPS/document_1/document_1.html#_Toc172623384"^^xsd:anyURI .

C1901A00006:411 a legcons:Item,
        skos:Concept,
        dcat:Resource ;
    rdfs:label "Item I411"@en-AU ;
    rdfs:comment "126 ALD  Power to ask questions - GraphNodeID: I411"@en-AU ;
    skos:definition "126 ALD  Power to ask questions"@en-AU ;
    skos:narrower C1901A00006:327 ;
    skos:prefLabel "Item I411"@en-AU ;
    dcat:accessURL "https://www.legislation.gov.au/C1901A00006/2024-07-01/2024-07-01/text/original/epub/OEBPS/document_1/document_1.html#_Toc172623385"^^xsd:anyURI .

C1901A00006:412 a legcons:Division,
        skos:Concept,
        dcat:Resource ;
    rdfs:label "Division D412"@en-AU ;
    rdfs:comment "Division 4 FAExportation of goods to Indonesia - GraphNodeID: D412"@en-AU ;
    skos:definition "Division 4 FAExportation of goods to Indonesia"@en-AU ;
    skos:narrower C1901A00006:305 ;
    skos:prefLabel "Division D412"@en-AU ;
    dcat:accessURL "https://www.legislation.gov.au/C1901A00006/2024-07-01/2024-07-01/text/original/epub/OEBPS/document_1/document_1.html#_Toc172623386"^^xsd:anyURI .

C1901A00006:413 a legcons:Item,
        skos:Concept,
        dcat:Resource ;
    rdfs:label "Item I413"@en-AU ;
    rdfs:comment "126 ALE  Definitions - GraphNodeID: I413"@en-AU ;
    skos:definition "126 ALE  Definitions"@en-AU ;
    skos:narrower C1901A00006:327 ;
    skos:prefLabel "Item I413"@en-AU ;
    dcat:accessURL "https://www.legislation.gov.au/C1901A00006/2024-07-01/2024-07-01/text/original/epub/OEBPS/document_1/document_1.html#_Toc172623387"^^xsd:anyURI .

C1901A00006:414 a legcons:Item,
        skos:Concept,
        dcat:Resource ;
    rdfs:label "Item I414"@en-AU ;
    rdfs:comment "126 ALF  Record keeping obligations - GraphNodeID: I414"@en-AU ;
    skos:definition "126 ALF  Record keeping obligations"@en-AU ;
    skos:narrower C1901A00006:327 ;
    skos:prefLabel "Item I414"@en-AU ;
    dcat:accessURL "https://www.legislation.gov.au/C1901A00006/2024-07-01/2024-07-01/text/original/epub/OEBPS/document_1/document_1.html#_Toc172623388"^^xsd:anyURI .

C1901A00006:415 a legcons:Item,
        skos:Concept,
        dcat:Resource ;
    rdfs:label "Item I415"@en-AU ;
    rdfs:comment "126 ALG  Power to require records - GraphNodeID: I415"@en-AU ;
    skos:definition "126 ALG  Power to require records"@en-AU ;
    skos:narrower C1901A00006:327 ;
    skos:prefLabel "Item I415"@en-AU ;
    dcat:accessURL "https://www.legislation.gov.au/C1901A00006/2024-07-01/2024-07-01/text/original/epub/OEBPS/document_1/document_1.html#_Toc172623389"^^xsd:anyURI .

C1901A00006:416 a legcons:Item,
        skos:Concept,
        dcat:Resource ;
    rdfs:label "Item I416"@en-AU ;
    rdfs:comment "126 ALH  Power to ask questions - GraphNodeID: I416"@en-AU ;
    skos:definition "126 ALH  Power to ask questions"@en-AU ;
    skos:narrower C1901A00006:327 ;
    skos:prefLabel "Item I416"@en-AU ;
    dcat:accessURL "https://www.legislation.gov.au/C1901A00006/2024-07-01/2024-07-01/text/original/epub/OEBPS/document_1/document_1.html#_Toc172623390"^^xsd:anyURI .

C1901A00006:417 a legcons:Division,
        skos:Concept,
        dcat:Resource ;
    rdfs:label "Division D417"@en-AU ;
    rdfs:comment "Division 4 GExportation of goods to Korea - GraphNodeID: D417"@en-AU ;
    skos:definition "Division 4 GExportation of goods to Korea"@en-AU ;
    skos:narrower C1901A00006:305 ;
    skos:prefLabel "Division D417"@en-AU ;
    dcat:accessURL "https://www.legislation.gov.au/C1901A00006/2024-07-01/2024-07-01/text/original/epub/OEBPS/document_1/document_1.html#_Toc172623391"^^xsd:anyURI .

C1901A00006:418 a legcons:Item,
        skos:Concept,
        dcat:Resource ;
    rdfs:label "Item I418"@en-AU ;
    rdfs:comment "126 AMA  Definitions - GraphNodeID: I418"@en-AU ;
    skos:definition "126 AMA  Definitions"@en-AU ;
    skos:narrower C1901A00006:327 ;
    skos:prefLabel "Item I418"@en-AU ;
    dcat:accessURL "https://www.legislation.gov.au/C1901A00006/2024-07-01/2024-07-01/text/original/epub/OEBPS/document_1/document_1.html#_Toc172623392"^^xsd:anyURI .

C1901A00006:419 a legcons:Item,
        skos:Concept,
        dcat:Resource ;
    rdfs:label "Item I419"@en-AU ;
    rdfs:comment "126 AMB  Record keeping obligations - GraphNodeID: I419"@en-AU ;
    skos:definition "126 AMB  Record keeping obligations"@en-AU ;
    skos:narrower C1901A00006:327 ;
    skos:prefLabel "Item I419"@en-AU ;
    dcat:accessURL "https://www.legislation.gov.au/C1901A00006/2024-07-01/2024-07-01/text/original/epub/OEBPS/document_1/document_1.html#_Toc172623393"^^xsd:anyURI .

C1901A00006:42 a legcons:Item,
        skos:Concept,
        dcat:Resource ;
    rdfs:label "Item I42"@en-AU ;
    rdfs:comment "34  No claim for compensation for loss - GraphNodeID: I42"@en-AU ;
    skos:definition "34  No claim for compensation for loss"@en-AU ;
    skos:narrower C1901A00006:33 ;
    skos:prefLabel "Item I42"@en-AU ;
    dcat:accessURL "https://www.legislation.gov.au/C1901A00006/2024-07-01/2024-07-01/text/original/epub/OEBPS/document_1/document_1.html#_Toc172623016"^^xsd:anyURI .

C1901A00006:420 a legcons:Item,
        skos:Concept,
        dcat:Resource ;
    rdfs:label "Item I420"@en-AU ;
    rdfs:comment "126 AMC  Power to require records - GraphNodeID: I420"@en-AU ;
    skos:definition "126 AMC  Power to require records"@en-AU ;
    skos:narrower C1901A00006:327 ;
    skos:prefLabel "Item I420"@en-AU ;
    dcat:accessURL "https://www.legislation.gov.au/C1901A00006/2024-07-01/2024-07-01/text/original/epub/OEBPS/document_1/document_1.html#_Toc172623394"^^xsd:anyURI .

C1901A00006:421 a legcons:Item,
        skos:Concept,
        dcat:Resource ;
    rdfs:label "Item I421"@en-AU ;
    rdfs:comment "126 AMD  Power to ask questions - GraphNodeID: I421"@en-AU ;
    skos:definition "126 AMD  Power to ask questions"@en-AU ;
    skos:narrower C1901A00006:327 ;
    skos:prefLabel "Item I421"@en-AU ;
    dcat:accessURL "https://www.legislation.gov.au/C1901A00006/2024-07-01/2024-07-01/text/original/epub/OEBPS/document_1/document_1.html#_Toc172623395"^^xsd:anyURI .

C1901A00006:422 a legcons:Division,
        skos:Concept,
        dcat:Resource ;
    rdfs:label "Division D422"@en-AU ;
    rdfs:comment "Division 4 GAExportation of goods to India - GraphNodeID: D422"@en-AU ;
    skos:definition "Division 4 GAExportation of goods to India"@en-AU ;
    skos:narrower C1901A00006:305 ;
    skos:prefLabel "Division D422"@en-AU ;
    dcat:accessURL "https://www.legislation.gov.au/C1901A00006/2024-07-01/2024-07-01/text/original/epub/OEBPS/document_1/document_1.html#_Toc172623396"^^xsd:anyURI .

C1901A00006:423 a legcons:Item,
        skos:Concept,
        dcat:Resource ;
    rdfs:label "Item I423"@en-AU ;
    rdfs:comment "126 AME  Definitions - GraphNodeID: I423"@en-AU ;
    skos:definition "126 AME  Definitions"@en-AU ;
    skos:narrower C1901A00006:327 ;
    skos:prefLabel "Item I423"@en-AU ;
    dcat:accessURL "https://www.legislation.gov.au/C1901A00006/2024-07-01/2024-07-01/text/original/epub/OEBPS/document_1/document_1.html#_Toc172623397"^^xsd:anyURI .

C1901A00006:424 a legcons:Item,
        skos:Concept,
        dcat:Resource ;
    rdfs:label "Item I424"@en-AU ;
    rdfs:comment "126 AMF  Record keeping obligations - GraphNodeID: I424"@en-AU ;
    skos:definition "126 AMF  Record keeping obligations"@en-AU ;
    skos:narrower C1901A00006:327 ;
    skos:prefLabel "Item I424"@en-AU ;
    dcat:accessURL "https://www.legislation.gov.au/C1901A00006/2024-07-01/2024-07-01/text/original/epub/OEBPS/document_1/document_1.html#_Toc172623398"^^xsd:anyURI .

C1901A00006:425 a legcons:Item,
        skos:Concept,
        dcat:Resource ;
    rdfs:label "Item I425"@en-AU ;
    rdfs:comment "126 AMG  Power to require records - GraphNodeID: I425"@en-AU ;
    skos:definition "126 AMG  Power to require records"@en-AU ;
    skos:narrower C1901A00006:327 ;
    skos:prefLabel "Item I425"@en-AU ;
    dcat:accessURL "https://www.legislation.gov.au/C1901A00006/2024-07-01/2024-07-01/text/original/epub/OEBPS/document_1/document_1.html#_Toc172623399"^^xsd:anyURI .

C1901A00006:426 a legcons:Item,
        skos:Concept,
        dcat:Resource ;
    rdfs:label "Item I426"@en-AU ;
    rdfs:comment "126 AMH  Power to ask questions - GraphNodeID: I426"@en-AU ;
    skos:definition "126 AMH  Power to ask questions"@en-AU ;
    skos:narrower C1901A00006:327 ;
    skos:prefLabel "Item I426"@en-AU ;
    dcat:accessURL "https://www.legislation.gov.au/C1901A00006/2024-07-01/2024-07-01/text/original/epub/OEBPS/document_1/document_1.html#_Toc172623400"^^xsd:anyURI .

C1901A00006:427 a legcons:Division,
        skos:Concept,
        dcat:Resource ;
    rdfs:label "Division D427"@en-AU ;
    rdfs:comment "Division 4 HExportation of goods to Japan - GraphNodeID: D427"@en-AU ;
    skos:definition "Division 4 HExportation of goods to Japan"@en-AU ;
    skos:narrower C1901A00006:305 ;
    skos:prefLabel "Division D427"@en-AU ;
    dcat:accessURL "https://www.legislation.gov.au/C1901A00006/2024-07-01/2024-07-01/text/original/epub/OEBPS/document_1/document_1.html#_Toc172623401"^^xsd:anyURI .

C1901A00006:428 a legcons:Item,
        skos:Concept,
        dcat:Resource ;
    rdfs:label "Item I428"@en-AU ;
    rdfs:comment "126 ANA  Definitions - GraphNodeID: I428"@en-AU ;
    skos:definition "126 ANA  Definitions"@en-AU ;
    skos:narrower C1901A00006:327 ;
    skos:prefLabel "Item I428"@en-AU ;
    dcat:accessURL "https://www.legislation.gov.au/C1901A00006/2024-07-01/2024-07-01/text/original/epub/OEBPS/document_1/document_1.html#_Toc172623402"^^xsd:anyURI .

C1901A00006:429 a legcons:Item,
        skos:Concept,
        dcat:Resource ;
    rdfs:label "Item I429"@en-AU ;
    rdfs:comment "126 ANB  Record keeping obligations - GraphNodeID: I429"@en-AU ;
    skos:definition "126 ANB  Record keeping obligations"@en-AU ;
    skos:narrower C1901A00006:327 ;
    skos:prefLabel "Item I429"@en-AU ;
    dcat:accessURL "https://www.legislation.gov.au/C1901A00006/2024-07-01/2024-07-01/text/original/epub/OEBPS/document_1/document_1.html#_Toc172623403"^^xsd:anyURI .

C1901A00006:43 a legcons:Item,
        skos:Concept,
        dcat:Resource ;
    rdfs:label "Item I43"@en-AU ;
    rdfs:comment "35  Goods imported by post - GraphNodeID: I43"@en-AU ;
    skos:definition "35  Goods imported by post"@en-AU ;
    skos:narrower C1901A00006:33 ;
    skos:prefLabel "Item I43"@en-AU ;
    dcat:accessURL "https://www.legislation.gov.au/C1901A00006/2024-07-01/2024-07-01/text/original/epub/OEBPS/document_1/document_1.html#_Toc172623017"^^xsd:anyURI .

C1901A00006:430 a legcons:Item,
        skos:Concept,
        dcat:Resource ;
    rdfs:label "Item I430"@en-AU ;
    rdfs:comment "126 ANC  Power to require records - GraphNodeID: I430"@en-AU ;
    skos:definition "126 ANC  Power to require records"@en-AU ;
    skos:narrower C1901A00006:327 ;
    skos:prefLabel "Item I430"@en-AU ;
    dcat:accessURL "https://www.legislation.gov.au/C1901A00006/2024-07-01/2024-07-01/text/original/epub/OEBPS/document_1/document_1.html#_Toc172623404"^^xsd:anyURI .

C1901A00006:431 a legcons:Item,
        skos:Concept,
        dcat:Resource ;
    rdfs:label "Item I431"@en-AU ;
    rdfs:comment "126 AND  Power to ask questions - GraphNodeID: I431"@en-AU ;
    skos:definition "126 AND  Power to ask questions"@en-AU ;
    skos:narrower C1901A00006:327 ;
    skos:prefLabel "Item I431"@en-AU ;
    dcat:accessURL "https://www.legislation.gov.au/C1901A00006/2024-07-01/2024-07-01/text/original/epub/OEBPS/document_1/document_1.html#_Toc172623405"^^xsd:anyURI .

C1901A00006:432 a legcons:Division,
        skos:Concept,
        dcat:Resource ;
    rdfs:label "Division D432"@en-AU ;
    rdfs:comment "Division 4 JExportation of goods to China - GraphNodeID: D432"@en-AU ;
    skos:definition "Division 4 JExportation of goods to China"@en-AU ;
    skos:narrower C1901A00006:305 ;
    skos:prefLabel "Division D432"@en-AU ;
    dcat:accessURL "https://www.legislation.gov.au/C1901A00006/2024-07-01/2024-07-01/text/original/epub/OEBPS/document_1/document_1.html#_Toc172623406"^^xsd:anyURI .

C1901A00006:433 a legcons:Item,
        skos:Concept,
        dcat:Resource ;
    rdfs:label "Item I433"@en-AU ;
    rdfs:comment "126 AOA  Definitions - GraphNodeID: I433"@en-AU ;
    skos:definition "126 AOA  Definitions"@en-AU ;
    skos:narrower C1901A00006:327 ;
    skos:prefLabel "Item I433"@en-AU ;
    dcat:accessURL "https://www.legislation.gov.au/C1901A00006/2024-07-01/2024-07-01/text/original/epub/OEBPS/document_1/document_1.html#_Toc172623407"^^xsd:anyURI .

C1901A00006:434 a legcons:Item,
        skos:Concept,
        dcat:Resource ;
    rdfs:label "Item I434"@en-AU ;
    rdfs:comment "126 AOB  Record keeping obligations - GraphNodeID: I434"@en-AU ;
    skos:definition "126 AOB  Record keeping obligations"@en-AU ;
    skos:narrower C1901A00006:327 ;
    skos:prefLabel "Item I434"@en-AU ;
    dcat:accessURL "https://www.legislation.gov.au/C1901A00006/2024-07-01/2024-07-01/text/original/epub/OEBPS/document_1/document_1.html#_Toc172623408"^^xsd:anyURI .

C1901A00006:435 a legcons:Item,
        skos:Concept,
        dcat:Resource ;
    rdfs:label "Item I435"@en-AU ;
    rdfs:comment "126 AOC  Power to require records - GraphNodeID: I435"@en-AU ;
    skos:definition "126 AOC  Power to require records"@en-AU ;
    skos:narrower C1901A00006:327 ;
    skos:prefLabel "Item I435"@en-AU ;
    dcat:accessURL "https://www.legislation.gov.au/C1901A00006/2024-07-01/2024-07-01/text/original/epub/OEBPS/document_1/document_1.html#_Toc172623409"^^xsd:anyURI .

C1901A00006:436 a legcons:Item,
        skos:Concept,
        dcat:Resource ;
    rdfs:label "Item I436"@en-AU ;
    rdfs:comment "126 AOD  Power to ask questions - GraphNodeID: I436"@en-AU ;
    skos:definition "126 AOD  Power to ask questions"@en-AU ;
    skos:narrower C1901A00006:327 ;
    skos:prefLabel "Item I436"@en-AU ;
    dcat:accessURL "https://www.legislation.gov.au/C1901A00006/2024-07-01/2024-07-01/text/original/epub/OEBPS/document_1/document_1.html#_Toc172623410"^^xsd:anyURI .

C1901A00006:437 a legcons:Division,
        skos:Concept,
        dcat:Resource ;
    rdfs:label "Division D437"@en-AU ;
    rdfs:comment "Division 4 KExportation of goods to Hong Kong China - GraphNodeID: D437"@en-AU ;
    skos:definition "Division 4 KExportation of goods to Hong Kong China"@en-AU ;
    skos:narrower C1901A00006:305 ;
    skos:prefLabel "Division D437"@en-AU ;
    dcat:accessURL "https://www.legislation.gov.au/C1901A00006/2024-07-01/2024-07-01/text/original/epub/OEBPS/document_1/document_1.html#_Toc172623411"^^xsd:anyURI .

C1901A00006:438 a legcons:Item,
        skos:Concept,
        dcat:Resource ;
    rdfs:label "Item I438"@en-AU ;
    rdfs:comment "126 APA  Definitions - GraphNodeID: I438"@en-AU ;
    skos:definition "126 APA  Definitions"@en-AU ;
    skos:narrower C1901A00006:327 ;
    skos:prefLabel "Item I438"@en-AU ;
    dcat:accessURL "https://www.legislation.gov.au/C1901A00006/2024-07-01/2024-07-01/text/original/epub/OEBPS/document_1/document_1.html#_Toc172623412"^^xsd:anyURI .

C1901A00006:439 a legcons:Item,
        skos:Concept,
        dcat:Resource ;
    rdfs:label "Item I439"@en-AU ;
    rdfs:comment "126 APB  Record keeping obligations - GraphNodeID: I439"@en-AU ;
    skos:definition "126 APB  Record keeping obligations"@en-AU ;
    skos:narrower C1901A00006:327 ;
    skos:prefLabel "Item I439"@en-AU ;
    dcat:accessURL "https://www.legislation.gov.au/C1901A00006/2024-07-01/2024-07-01/text/original/epub/OEBPS/document_1/document_1.html#_Toc172623413"^^xsd:anyURI .

C1901A00006:44 a legcons:Item,
        skos:Concept,
        dcat:Resource ;
    rdfs:label "Item I44"@en-AU ;
    rdfs:comment "35 A  Amount payable for failure to keep dutiable goods safely etc - GraphNodeID: I44"@en-AU ;
    skos:definition "35 A  Amount payable for failure to keep dutiable goods safely etc"@en-AU ;
    skos:narrower C1901A00006:33 ;
    skos:prefLabel "Item I44"@en-AU ;
    dcat:accessURL "https://www.legislation.gov.au/C1901A00006/2024-07-01/2024-07-01/text/original/epub/OEBPS/document_1/document_1.html#_Toc172623018"^^xsd:anyURI .

C1901A00006:440 a legcons:Item,
        skos:Concept,
        dcat:Resource ;
    rdfs:label "Item I440"@en-AU ;
    rdfs:comment "126 APC  Power to require records - GraphNodeID: I440"@en-AU ;
    skos:definition "126 APC  Power to require records"@en-AU ;
    skos:narrower C1901A00006:327 ;
    skos:prefLabel "Item I440"@en-AU ;
    dcat:accessURL "https://www.legislation.gov.au/C1901A00006/2024-07-01/2024-07-01/text/original/epub/OEBPS/document_1/document_1.html#_Toc172623414"^^xsd:anyURI .

C1901A00006:441 a legcons:Item,
        skos:Concept,
        dcat:Resource ;
    rdfs:label "Item I441"@en-AU ;
    rdfs:comment "126 APD  Power to ask questions - GraphNodeID: I441"@en-AU ;
    skos:definition "126 APD  Power to ask questions"@en-AU ;
    skos:narrower C1901A00006:327 ;
    skos:prefLabel "Item I441"@en-AU ;
    dcat:accessURL "https://www.legislation.gov.au/C1901A00006/2024-07-01/2024-07-01/text/original/epub/OEBPS/document_1/document_1.html#_Toc172623415"^^xsd:anyURI .

C1901A00006:442 a legcons:Division,
        skos:Concept,
        dcat:Resource ;
    rdfs:label "Division D442"@en-AU ;
    rdfs:comment "Division 4 LExportation of goods to Parties to the Regional Comprehensive Economic Partnership Agreement - GraphNodeID: D442"@en-AU ;
    skos:definition "Division 4 LExportation of goods to Parties to the Regional Comprehensive Economic Partnership Agreement"@en-AU ;
    skos:narrower C1901A00006:305 ;
    skos:prefLabel "Division D442"@en-AU ;
    dcat:accessURL "https://www.legislation.gov.au/C1901A00006/2024-07-01/2024-07-01/text/original/epub/OEBPS/document_1/document_1.html#_Toc172623416"^^xsd:anyURI .

C1901A00006:443 a legcons:Item,
        skos:Concept,
        dcat:Resource ;
    rdfs:label "Item I443"@en-AU ;
    rdfs:comment "126 AQA  Definitions - GraphNodeID: I443"@en-AU ;
    skos:definition "126 AQA  Definitions"@en-AU ;
    skos:narrower C1901A00006:327 ;
    skos:prefLabel "Item I443"@en-AU ;
    dcat:accessURL "https://www.legislation.gov.au/C1901A00006/2024-07-01/2024-07-01/text/original/epub/OEBPS/document_1/document_1.html#_Toc172623417"^^xsd:anyURI .

C1901A00006:444 a legcons:Item,
        skos:Concept,
        dcat:Resource ;
    rdfs:label "Item I444"@en-AU ;
    rdfs:comment "126 AQB  Record keeping obligations - GraphNodeID: I444"@en-AU ;
    skos:definition "126 AQB  Record keeping obligations"@en-AU ;
    skos:narrower C1901A00006:327 ;
    skos:prefLabel "Item I444"@en-AU ;
    dcat:accessURL "https://www.legislation.gov.au/C1901A00006/2024-07-01/2024-07-01/text/original/epub/OEBPS/document_1/document_1.html#_Toc172623418"^^xsd:anyURI .

C1901A00006:445 a legcons:Item,
        skos:Concept,
        dcat:Resource ;
    rdfs:label "Item I445"@en-AU ;
    rdfs:comment "126 AQC  Power to require records - GraphNodeID: I445"@en-AU ;
    skos:definition "126 AQC  Power to require records"@en-AU ;
    skos:narrower C1901A00006:327 ;
    skos:prefLabel "Item I445"@en-AU ;
    dcat:accessURL "https://www.legislation.gov.au/C1901A00006/2024-07-01/2024-07-01/text/original/epub/OEBPS/document_1/document_1.html#_Toc172623419"^^xsd:anyURI .

C1901A00006:446 a legcons:Item,
        skos:Concept,
        dcat:Resource ;
    rdfs:label "Item I446"@en-AU ;
    rdfs:comment "126 AQD  Power to ask questions - GraphNodeID: I446"@en-AU ;
    skos:definition "126 AQD  Power to ask questions"@en-AU ;
    skos:narrower C1901A00006:327 ;
    skos:prefLabel "Item I446"@en-AU ;
    dcat:accessURL "https://www.legislation.gov.au/C1901A00006/2024-07-01/2024-07-01/text/original/epub/OEBPS/document_1/document_1.html#_Toc172623420"^^xsd:anyURI .

C1901A00006:447 a legcons:Division,
        skos:Concept,
        dcat:Resource ;
    rdfs:label "Division D447"@en-AU ;
    rdfs:comment "Division 4 MExportation of goods to the United Kingdom - GraphNodeID: D447"@en-AU ;
    skos:definition "Division 4 MExportation of goods to the United Kingdom"@en-AU ;
    skos:narrower C1901A00006:305 ;
    skos:prefLabel "Division D447"@en-AU ;
    dcat:accessURL "https://www.legislation.gov.au/C1901A00006/2024-07-01/2024-07-01/text/original/epub/OEBPS/document_1/document_1.html#_Toc172623421"^^xsd:anyURI .

C1901A00006:448 a legcons:Item,
        skos:Concept,
        dcat:Resource ;
    rdfs:label "Item I448"@en-AU ;
    rdfs:comment "126 ARA  Definitions - GraphNodeID: I448"@en-AU ;
    skos:definition "126 ARA  Definitions"@en-AU ;
    skos:narrower C1901A00006:327 ;
    skos:prefLabel "Item I448"@en-AU ;
    dcat:accessURL "https://www.legislation.gov.au/C1901A00006/2024-07-01/2024-07-01/text/original/epub/OEBPS/document_1/document_1.html#_Toc172623422"^^xsd:anyURI .

C1901A00006:449 a legcons:Item,
        skos:Concept,
        dcat:Resource ;
    rdfs:label "Item I449"@en-AU ;
    rdfs:comment "126 ARB  Record keeping obligations - GraphNodeID: I449"@en-AU ;
    skos:definition "126 ARB  Record keeping obligations"@en-AU ;
    skos:narrower C1901A00006:327 ;
    skos:prefLabel "Item I449"@en-AU ;
    dcat:accessURL "https://www.legislation.gov.au/C1901A00006/2024-07-01/2024-07-01/text/original/epub/OEBPS/document_1/document_1.html#_Toc172623423"^^xsd:anyURI .

C1901A00006:45 a legcons:Item,
        skos:Concept,
        dcat:Resource ;
    rdfs:label "Item I45"@en-AU ;
    rdfs:comment "36  Offences for failure to keep goods safely or failure to account for goods - GraphNodeID: I45"@en-AU ;
    skos:definition "36  Offences for failure to keep goods safely or failure to account for goods"@en-AU ;
    skos:narrower C1901A00006:33 ;
    skos:prefLabel "Item I45"@en-AU ;
    dcat:accessURL "https://www.legislation.gov.au/C1901A00006/2024-07-01/2024-07-01/text/original/epub/OEBPS/document_1/document_1.html#_Toc172623019"^^xsd:anyURI .

C1901A00006:450 a legcons:Item,
        skos:Concept,
        dcat:Resource ;
    rdfs:label "Item I450"@en-AU ;
    rdfs:comment "126 ARC  Power to require records - GraphNodeID: I450"@en-AU ;
    skos:definition "126 ARC  Power to require records"@en-AU ;
    skos:narrower C1901A00006:327 ;
    skos:prefLabel "Item I450"@en-AU ;
    dcat:accessURL "https://www.legislation.gov.au/C1901A00006/2024-07-01/2024-07-01/text/original/epub/OEBPS/document_1/document_1.html#_Toc172623424"^^xsd:anyURI .

C1901A00006:451 a legcons:Item,
        skos:Concept,
        dcat:Resource ;
    rdfs:label "Item I451"@en-AU ;
    rdfs:comment "126 ARD  Power to ask questions - GraphNodeID: I451"@en-AU ;
    skos:definition "126 ARD  Power to ask questions"@en-AU ;
    skos:narrower C1901A00006:327 ;
    skos:prefLabel "Item I451"@en-AU ;
    dcat:accessURL "https://www.legislation.gov.au/C1901A00006/2024-07-01/2024-07-01/text/original/epub/OEBPS/document_1/document_1.html#_Toc172623425"^^xsd:anyURI .

C1901A00006:452 a legcons:Division,
        skos:Concept,
        dcat:Resource ;
    rdfs:label "Division D452"@en-AU ;
    rdfs:comment "Division 5 Miscellaneous - GraphNodeID: D452"@en-AU ;
    skos:definition "Division 5 Miscellaneous"@en-AU ;
    skos:narrower C1901A00006:305 ;
    skos:prefLabel "Division D452"@en-AU ;
    dcat:accessURL "https://www.legislation.gov.au/C1901A00006/2024-07-01/2024-07-01/text/original/epub/OEBPS/document_1/document_1.html#_Toc172623426"^^xsd:anyURI .

C1901A00006:453 a legcons:Item,
        skos:Concept,
        dcat:Resource ;
    rdfs:label "Item I453"@en-AU ;
    rdfs:comment "126 A  Export of installations - GraphNodeID: I453"@en-AU ;
    skos:definition "126 A  Export of installations"@en-AU ;
    skos:narrower C1901A00006:327 ;
    skos:prefLabel "Item I453"@en-AU ;
    dcat:accessURL "https://www.legislation.gov.au/C1901A00006/2024-07-01/2024-07-01/text/original/epub/OEBPS/document_1/document_1.html#_Toc172623427"^^xsd:anyURI .

C1901A00006:454 a legcons:Item,
        skos:Concept,
        dcat:Resource ;
    rdfs:label "Item I454"@en-AU ;
    rdfs:comment "126 B  Export of goods from installations - GraphNodeID: I454"@en-AU ;
    skos:definition "126 B  Export of goods from installations"@en-AU ;
    skos:narrower C1901A00006:327 ;
    skos:prefLabel "Item I454"@en-AU ;
    dcat:accessURL "https://www.legislation.gov.au/C1901A00006/2024-07-01/2024-07-01/text/original/epub/OEBPS/document_1/document_1.html#_Toc172623428"^^xsd:anyURI .

C1901A00006:455 a legcons:Item,
        skos:Concept,
        dcat:Resource ;
    rdfs:label "Item I455"@en-AU ;
    rdfs:comment "126 C  Size of exporting vessel - GraphNodeID: I455"@en-AU ;
    skos:definition "126 C  Size of exporting vessel"@en-AU ;
    skos:narrower C1901A00006:327 ;
    skos:prefLabel "Item I455"@en-AU ;
    dcat:accessURL "https://www.legislation.gov.au/C1901A00006/2024-07-01/2024-07-01/text/original/epub/OEBPS/document_1/document_1.html#_Toc172623429"^^xsd:anyURI .

C1901A00006:457 a legcons:Part,
        skos:Concept,
        dcat:Resource ;
    rdfs:label "Part P457"@en-AU ;
    rdfs:comment "Part VIAElectronic communications - GraphNodeID: P457"@en-AU ;
    skos:definition "Part VIAElectronic communications"@en-AU ;
    skos:narrower C1901A00006:456 ;
    skos:prefLabel "Part P457"@en-AU ;
    dcat:accessURL "https://www.legislation.gov.au/C1901A00006/2024-07-01/2024-07-01/text/original/epub/OEBPS/document_2/document_2.html#_Toc172624212"^^xsd:anyURI .

C1901A00006:458 a legcons:Item,
        skos:Concept,
        dcat:Resource ;
    rdfs:label "Item I458"@en-AU ;
    rdfs:comment "126 D  Comptroller General of Customs to maintain information systems - GraphNodeID: I458"@en-AU ;
    skos:definition "126 D  Comptroller General of Customs to maintain information systems"@en-AU ;
    skos:narrower C1901A00006:327 ;
    skos:prefLabel "Item I458"@en-AU ;
    dcat:accessURL "https://www.legislation.gov.au/C1901A00006/2024-07-01/2024-07-01/text/original/epub/OEBPS/document_2/document_2.html#_Toc172624213"^^xsd:anyURI .

C1901A00006:459 a legcons:Item,
        skos:Concept,
        dcat:Resource ;
    rdfs:label "Item I459"@en-AU ;
    rdfs:comment "126 DA  Communications standards and operation - GraphNodeID: I459"@en-AU ;
    skos:definition "126 DA  Communications standards and operation"@en-AU ;
    skos:narrower C1901A00006:327 ;
    skos:prefLabel "Item I459"@en-AU ;
    dcat:accessURL "https://www.legislation.gov.au/C1901A00006/2024-07-01/2024-07-01/text/original/epub/OEBPS/document_2/document_2.html#_Toc172624214"^^xsd:anyURI .

C1901A00006:46 a legcons:Item,
        skos:Concept,
        dcat:Resource ;
    rdfs:label "Item I46"@en-AU ;
    rdfs:comment "37  Accounting for goods - GraphNodeID: I46"@en-AU ;
    skos:definition "37  Accounting for goods"@en-AU ;
    skos:narrower C1901A00006:33 ;
    skos:prefLabel "Item I46"@en-AU ;
    dcat:accessURL "https://www.legislation.gov.au/C1901A00006/2024-07-01/2024-07-01/text/original/epub/OEBPS/document_1/document_1.html#_Toc172623020"^^xsd:anyURI .

C1901A00006:460 a legcons:Item,
        skos:Concept,
        dcat:Resource ;
    rdfs:label "Item I460"@en-AU ;
    rdfs:comment "126 DB  Authentication of certain electronic communications - GraphNodeID: I460"@en-AU ;
    skos:definition "126 DB  Authentication of certain electronic communications"@en-AU ;
    skos:narrower C1901A00006:327 ;
    skos:prefLabel "Item I460"@en-AU ;
    dcat:accessURL "https://www.legislation.gov.au/C1901A00006/2024-07-01/2024-07-01/text/original/epub/OEBPS/document_2/document_2.html#_Toc172624215"^^xsd:anyURI .

C1901A00006:461 a legcons:Item,
        skos:Concept,
        dcat:Resource ;
    rdfs:label "Item I461"@en-AU ;
    rdfs:comment "126 DC  Records of certain electronic communications - GraphNodeID: I461"@en-AU ;
    skos:definition "126 DC  Records of certain electronic communications"@en-AU ;
    skos:narrower C1901A00006:327 ;
    skos:prefLabel "Item I461"@en-AU ;
    dcat:accessURL "https://www.legislation.gov.au/C1901A00006/2024-07-01/2024-07-01/text/original/epub/OEBPS/document_2/document_2.html#_Toc172624216"^^xsd:anyURI .

C1901A00006:462 a legcons:Item,
        skos:Concept,
        dcat:Resource ;
    rdfs:label "Item I462"@en-AU ;
    rdfs:comment "126 DD  Authentication records and Electronic Transactions Act 1999 - GraphNodeID: I462"@en-AU ;
    skos:definition "126 DD  Authentication records and Electronic Transactions Act 1999"@en-AU ;
    skos:narrower C1901A00006:327 ;
    skos:prefLabel "Item I462"@en-AU ;
    dcat:accessURL "https://www.legislation.gov.au/C1901A00006/2024-07-01/2024-07-01/text/original/epub/OEBPS/document_2/document_2.html#_Toc172624217"^^xsd:anyURI .

C1901A00006:463 a legcons:Item,
        skos:Concept,
        dcat:Resource ;
    rdfs:label "Item I463"@en-AU ;
    rdfs:comment "126 E  Communication to Department when information system is temporarily inoperative - GraphNodeID: I463"@en-AU ;
    skos:definition "126 E  Communication to Department when information system is temporarily inoperative"@en-AU ;
    skos:narrower C1901A00006:327 ;
    skos:prefLabel "Item I463"@en-AU ;
    dcat:accessURL "https://www.legislation.gov.au/C1901A00006/2024-07-01/2024-07-01/text/original/epub/OEBPS/document_2/document_2.html#_Toc172624218"^^xsd:anyURI .

C1901A00006:464 a legcons:Item,
        skos:Concept,
        dcat:Resource ;
    rdfs:label "Item I464"@en-AU ;
    rdfs:comment "126 F  Payment when information system is temporarily inoperative - GraphNodeID: I464"@en-AU ;
    skos:definition "126 F  Payment when information system is temporarily inoperative"@en-AU ;
    skos:narrower C1901A00006:327 ;
    skos:prefLabel "Item I464"@en-AU ;
    dcat:accessURL "https://www.legislation.gov.au/C1901A00006/2024-07-01/2024-07-01/text/original/epub/OEBPS/document_2/document_2.html#_Toc172624219"^^xsd:anyURI .

C1901A00006:465 a legcons:Item,
        skos:Concept,
        dcat:Resource ;
    rdfs:label "Item I465"@en-AU ;
    rdfs:comment "126 G  Meaning of temporarily inoperative - GraphNodeID: I465"@en-AU ;
    skos:definition "126 G  Meaning of temporarily inoperative"@en-AU ;
    skos:narrower C1901A00006:327 ;
    skos:prefLabel "Item I465"@en-AU ;
    dcat:accessURL "https://www.legislation.gov.au/C1901A00006/2024-07-01/2024-07-01/text/original/epub/OEBPS/document_2/document_2.html#_Toc172624220"^^xsd:anyURI .

C1901A00006:466 a legcons:Item,
        skos:Concept,
        dcat:Resource ;
    rdfs:label "Item I466"@en-AU ;
    rdfs:comment "126 H  Comptroller General of Customs may arrange for use of computer programs to make decisions etc - GraphNodeID: I466"@en-AU ;
    skos:definition "126 H  Comptroller General of Customs may arrange for use of computer programs to make decisions etc"@en-AU ;
    skos:narrower C1901A00006:327 ;
    skos:prefLabel "Item I466"@en-AU ;
    dcat:accessURL "https://www.legislation.gov.au/C1901A00006/2024-07-01/2024-07-01/text/original/epub/OEBPS/document_2/document_2.html#_Toc172624221"^^xsd:anyURI .

C1901A00006:467 a legcons:Part,
        skos:Concept,
        dcat:Resource ;
    rdfs:label "Part P467"@en-AU ;
    rdfs:comment "Part VIIShips stores and aircrafts stores - GraphNodeID: P467"@en-AU ;
    skos:definition "Part VIIShips stores and aircrafts stores"@en-AU ;
    skos:narrower C1901A00006:456 ;
    skos:prefLabel "Part P467"@en-AU ;
    dcat:accessURL "https://www.legislation.gov.au/C1901A00006/2024-07-01/2024-07-01/text/original/epub/OEBPS/document_2/document_2.html#_Toc172624222"^^xsd:anyURI .

C1901A00006:468 a legcons:Item,
        skos:Concept,
        dcat:Resource ;
    rdfs:label "Item I468"@en-AU ;
    rdfs:comment "127  Use of ships and aircrafts stores - GraphNodeID: I468"@en-AU ;
    skos:definition "127  Use of ships and aircrafts stores"@en-AU ;
    skos:narrower C1901A00006:327 ;
    skos:prefLabel "Item I468"@en-AU ;
    dcat:accessURL "https://www.legislation.gov.au/C1901A00006/2024-07-01/2024-07-01/text/original/epub/OEBPS/document_2/document_2.html#_Toc172624223"^^xsd:anyURI .

C1901A00006:469 a legcons:Item,
        skos:Concept,
        dcat:Resource ;
    rdfs:label "Item I469"@en-AU ;
    rdfs:comment "128  Unshipment of ships and aircrafts stores - GraphNodeID: I469"@en-AU ;
    skos:definition "128  Unshipment of ships and aircrafts stores"@en-AU ;
    skos:narrower C1901A00006:327 ;
    skos:prefLabel "Item I469"@en-AU ;
    dcat:accessURL "https://www.legislation.gov.au/C1901A00006/2024-07-01/2024-07-01/text/original/epub/OEBPS/document_2/document_2.html#_Toc172624224"^^xsd:anyURI .

C1901A00006:47 a legcons:Item,
        skos:Concept,
        dcat:Resource ;
    rdfs:label "Item I47"@en-AU ;
    rdfs:comment "42  Right to require security - GraphNodeID: I47"@en-AU ;
    skos:definition "42  Right to require security"@en-AU ;
    skos:narrower C1901A00006:33 ;
    skos:prefLabel "Item I47"@en-AU ;
    dcat:accessURL "https://www.legislation.gov.au/C1901A00006/2024-07-01/2024-07-01/text/original/epub/OEBPS/document_1/document_1.html#_Toc172623021"^^xsd:anyURI .

C1901A00006:470 a legcons:Item,
        skos:Concept,
        dcat:Resource ;
    rdfs:label "Item I470"@en-AU ;
    rdfs:comment "129  Ships and aircrafts stores not to be taken on board without approval - GraphNodeID: I470"@en-AU ;
    skos:definition "129  Ships and aircrafts stores not to be taken on board without approval"@en-AU ;
    skos:narrower C1901A00006:327 ;
    skos:prefLabel "Item I470"@en-AU ;
    dcat:accessURL "https://www.legislation.gov.au/C1901A00006/2024-07-01/2024-07-01/text/original/epub/OEBPS/document_2/document_2.html#_Toc172624225"^^xsd:anyURI .

C1901A00006:471 a legcons:Item,
        skos:Concept,
        dcat:Resource ;
    rdfs:label "Item I471"@en-AU ;
    rdfs:comment "130  Ships and aircrafts stores exempt from duty - GraphNodeID: I471"@en-AU ;
    skos:definition "130  Ships and aircrafts stores exempt from duty"@en-AU ;
    skos:narrower C1901A00006:327 ;
    skos:prefLabel "Item I471"@en-AU ;
    dcat:accessURL "https://www.legislation.gov.au/C1901A00006/2024-07-01/2024-07-01/text/original/epub/OEBPS/document_2/document_2.html#_Toc172624226"^^xsd:anyURI .

C1901A00006:472 a legcons:Item,
        skos:Concept,
        dcat:Resource ;
    rdfs:label "Item I472"@en-AU ;
    rdfs:comment "130 A  Entry not required for ships or aircrafts stores - GraphNodeID: I472"@en-AU ;
    skos:definition "130 A  Entry not required for ships or aircrafts stores"@en-AU ;
    skos:narrower C1901A00006:327 ;
    skos:prefLabel "Item I472"@en-AU ;
    dcat:accessURL "https://www.legislation.gov.au/C1901A00006/2024-07-01/2024-07-01/text/original/epub/OEBPS/document_2/document_2.html#_Toc172624227"^^xsd:anyURI .

C1901A00006:473 a legcons:Item,
        skos:Concept,
        dcat:Resource ;
    rdfs:label "Item I473"@en-AU ;
    rdfs:comment "130 B  Payment of duty on ships or aircrafts stores - GraphNodeID: I473"@en-AU ;
    skos:definition "130 B  Payment of duty on ships or aircrafts stores"@en-AU ;
    skos:narrower C1901A00006:327 ;
    skos:prefLabel "Item I473"@en-AU ;
    dcat:accessURL "https://www.legislation.gov.au/C1901A00006/2024-07-01/2024-07-01/text/original/epub/OEBPS/document_2/document_2.html#_Toc172624228"^^xsd:anyURI .

C1901A00006:474 a legcons:Item,
        skos:Concept,
        dcat:Resource ;
    rdfs:label "Item I474"@en-AU ;
    rdfs:comment "130 C  Interpretation - GraphNodeID: I474"@en-AU ;
    skos:definition "130 C  Interpretation"@en-AU ;
    skos:narrower C1901A00006:327 ;
    skos:prefLabel "Item I474"@en-AU ;
    dcat:accessURL "https://www.legislation.gov.au/C1901A00006/2024-07-01/2024-07-01/text/original/epub/OEBPS/document_2/document_2.html#_Toc172624229"^^xsd:anyURI .

C1901A00006:476 a legcons:Division,
        skos:Concept,
        dcat:Resource ;
    rdfs:label "Division D476"@en-AU ;
    rdfs:comment "Division 1 The payment and computation of duties generally - GraphNodeID: D476"@en-AU ;
    skos:definition "Division 1 The payment and computation of duties generally"@en-AU ;
    skos:narrower C1901A00006:475 ;
    skos:prefLabel "Division D476"@en-AU ;
    dcat:accessURL "https://www.legislation.gov.au/C1901A00006/2024-07-01/2024-07-01/text/original/epub/OEBPS/document_2/document_2.html#_Toc172624231"^^xsd:anyURI .

C1901A00006:477 a legcons:Item,
        skos:Concept,
        dcat:Resource ;
    rdfs:label "Item I477"@en-AU ;
    rdfs:comment "131 A  Fish caught by Australian ships - GraphNodeID: I477"@en-AU ;
    skos:definition "131 A  Fish caught by Australian ships"@en-AU ;
    skos:narrower C1901A00006:327 ;
    skos:prefLabel "Item I477"@en-AU ;
    dcat:accessURL "https://www.legislation.gov.au/C1901A00006/2024-07-01/2024-07-01/text/original/epub/OEBPS/document_2/document_2.html#_Toc172624232"^^xsd:anyURI .

C1901A00006:478 a legcons:Item,
        skos:Concept,
        dcat:Resource ;
    rdfs:label "Item I478"@en-AU ;
    rdfs:comment "131 AA  No duty on goods for Timor Sea petroleum activities purpose - GraphNodeID: I478"@en-AU ;
    skos:definition "131 AA  No duty on goods for Timor Sea petroleum activities purpose"@en-AU ;
    skos:narrower C1901A00006:327 ;
    skos:prefLabel "Item I478"@en-AU ;
    dcat:accessURL "https://www.legislation.gov.au/C1901A00006/2024-07-01/2024-07-01/text/original/epub/OEBPS/document_2/document_2.html#_Toc172624233"^^xsd:anyURI .

C1901A00006:479 a legcons:Item,
        skos:Concept,
        dcat:Resource ;
    rdfs:label "Item I479"@en-AU ;
    rdfs:comment "131 B  Liability of Commonwealth authorities to pay duties of Customs - GraphNodeID: I479"@en-AU ;
    skos:definition "131 B  Liability of Commonwealth authorities to pay duties of Customs"@en-AU ;
    skos:narrower C1901A00006:327 ;
    skos:prefLabel "Item I479"@en-AU ;
    dcat:accessURL "https://www.legislation.gov.au/C1901A00006/2024-07-01/2024-07-01/text/original/epub/OEBPS/document_2/document_2.html#_Toc172624234"^^xsd:anyURI .

C1901A00006:48 a legcons:Item,
        skos:Concept,
        dcat:Resource ;
    rdfs:label "Item I48"@en-AU ;
    rdfs:comment "43  Form of security - GraphNodeID: I48"@en-AU ;
    skos:definition "43  Form of security"@en-AU ;
    skos:narrower C1901A00006:33 ;
    skos:prefLabel "Item I48"@en-AU ;
    dcat:accessURL "https://www.legislation.gov.au/C1901A00006/2024-07-01/2024-07-01/text/original/epub/OEBPS/document_1/document_1.html#_Toc172623022"^^xsd:anyURI .

C1901A00006:480 a legcons:Item,
        skos:Concept,
        dcat:Resource ;
    rdfs:label "Item I480"@en-AU ;
    rdfs:comment "132  Rate of import duty - GraphNodeID: I480"@en-AU ;
    skos:definition "132  Rate of import duty"@en-AU ;
    skos:narrower C1901A00006:327 ;
    skos:prefLabel "Item I480"@en-AU ;
    dcat:accessURL "https://www.legislation.gov.au/C1901A00006/2024-07-01/2024-07-01/text/original/epub/OEBPS/document_2/document_2.html#_Toc172624235"^^xsd:anyURI .

C1901A00006:481 a legcons:Item,
        skos:Concept,
        dcat:Resource ;
    rdfs:label "Item I481"@en-AU ;
    rdfs:comment "132 AA  When import duty must be paid - GraphNodeID: I481"@en-AU ;
    skos:definition "132 AA  When import duty must be paid"@en-AU ;
    skos:narrower C1901A00006:327 ;
    skos:prefLabel "Item I481"@en-AU ;
    dcat:accessURL "https://www.legislation.gov.au/C1901A00006/2024-07-01/2024-07-01/text/original/epub/OEBPS/document_2/document_2.html#_Toc172624236"^^xsd:anyURI .

C1901A00006:482 a legcons:Item,
        skos:Concept,
        dcat:Resource ;
    rdfs:label "Item I482"@en-AU ;
    rdfs:comment "132 A  Prepayment of duty - GraphNodeID: I482"@en-AU ;
    skos:definition "132 A  Prepayment of duty"@en-AU ;
    skos:narrower C1901A00006:327 ;
    skos:prefLabel "Item I482"@en-AU ;
    dcat:accessURL "https://www.legislation.gov.au/C1901A00006/2024-07-01/2024-07-01/text/original/epub/OEBPS/document_2/document_2.html#_Toc172624237"^^xsd:anyURI .

C1901A00006:483 a legcons:Item,
        skos:Concept,
        dcat:Resource ;
    rdfs:label "Item I483"@en-AU ;
    rdfs:comment "132 B  Declared period quotaseffect on rates of import duty - GraphNodeID: I483"@en-AU ;
    skos:definition "132 B  Declared period quotaseffect on rates of import duty"@en-AU ;
    skos:narrower C1901A00006:327 ;
    skos:prefLabel "Item I483"@en-AU ;
    dcat:accessURL "https://www.legislation.gov.au/C1901A00006/2024-07-01/2024-07-01/text/original/epub/OEBPS/document_2/document_2.html#_Toc172624238"^^xsd:anyURI .

C1901A00006:484 a legcons:Item,
        skos:Concept,
        dcat:Resource ;
    rdfs:label "Item I484"@en-AU ;
    rdfs:comment "132 C  Revocation and variation of quota orders - GraphNodeID: I484"@en-AU ;
    skos:definition "132 C  Revocation and variation of quota orders"@en-AU ;
    skos:narrower C1901A00006:327 ;
    skos:prefLabel "Item I484"@en-AU ;
    dcat:accessURL "https://www.legislation.gov.au/C1901A00006/2024-07-01/2024-07-01/text/original/epub/OEBPS/document_2/document_2.html#_Toc172624239"^^xsd:anyURI .

C1901A00006:485 a legcons:Item,
        skos:Concept,
        dcat:Resource ;
    rdfs:label "Item I485"@en-AU ;
    rdfs:comment "132 D  Service of quota orders etc - GraphNodeID: I485"@en-AU ;
    skos:definition "132 D  Service of quota orders etc"@en-AU ;
    skos:narrower C1901A00006:327 ;
    skos:prefLabel "Item I485"@en-AU ;
    dcat:accessURL "https://www.legislation.gov.au/C1901A00006/2024-07-01/2024-07-01/text/original/epub/OEBPS/document_2/document_2.html#_Toc172624240"^^xsd:anyURI .

C1901A00006:486 a legcons:Item,
        skos:Concept,
        dcat:Resource ;
    rdfs:label "Item I486"@en-AU ;
    rdfs:comment "133  Export duties - GraphNodeID: I486"@en-AU ;
    skos:definition "133  Export duties"@en-AU ;
    skos:narrower C1901A00006:327 ;
    skos:prefLabel "Item I486"@en-AU ;
    dcat:accessURL "https://www.legislation.gov.au/C1901A00006/2024-07-01/2024-07-01/text/original/epub/OEBPS/document_2/document_2.html#_Toc172624241"^^xsd:anyURI .

C1901A00006:487 a legcons:Item,
        skos:Concept,
        dcat:Resource ;
    rdfs:label "Item I487"@en-AU ;
    rdfs:comment "134  Weights and measures - GraphNodeID: I487"@en-AU ;
    skos:definition "134  Weights and measures"@en-AU ;
    skos:narrower C1901A00006:327 ;
    skos:prefLabel "Item I487"@en-AU ;
    dcat:accessURL "https://www.legislation.gov.au/C1901A00006/2024-07-01/2024-07-01/text/original/epub/OEBPS/document_2/document_2.html#_Toc172624242"^^xsd:anyURI .

C1901A00006:488 a legcons:Item,
        skos:Concept,
        dcat:Resource ;
    rdfs:label "Item I488"@en-AU ;
    rdfs:comment "135  Proportion - GraphNodeID: I488"@en-AU ;
    skos:definition "135  Proportion"@en-AU ;
    skos:narrower C1901A00006:327 ;
    skos:prefLabel "Item I488"@en-AU ;
    dcat:accessURL "https://www.legislation.gov.au/C1901A00006/2024-07-01/2024-07-01/text/original/epub/OEBPS/document_2/document_2.html#_Toc172624243"^^xsd:anyURI .

C1901A00006:489 a legcons:Item,
        skos:Concept,
        dcat:Resource ;
    rdfs:label "Item I489"@en-AU ;
    rdfs:comment "136  Manner of fixing duty - GraphNodeID: I489"@en-AU ;
    skos:definition "136  Manner of fixing duty"@en-AU ;
    skos:narrower C1901A00006:327 ;
    skos:prefLabel "Item I489"@en-AU ;
    dcat:accessURL "https://www.legislation.gov.au/C1901A00006/2024-07-01/2024-07-01/text/original/epub/OEBPS/document_2/document_2.html#_Toc172624244"^^xsd:anyURI .

C1901A00006:49 a legcons:Item,
        skos:Concept,
        dcat:Resource ;
    rdfs:label "Item I49"@en-AU ;
    rdfs:comment "44  General securities may be given - GraphNodeID: I49"@en-AU ;
    skos:definition "44  General securities may be given"@en-AU ;
    skos:narrower C1901A00006:33 ;
    skos:prefLabel "Item I49"@en-AU ;
    dcat:accessURL "https://www.legislation.gov.au/C1901A00006/2024-07-01/2024-07-01/text/original/epub/OEBPS/document_1/document_1.html#_Toc172623023"^^xsd:anyURI .

C1901A00006:490 a legcons:Item,
        skos:Concept,
        dcat:Resource ;
    rdfs:label "Item I490"@en-AU ;
    rdfs:comment "137  Manner of determining volumes of and fixing duty on beer - GraphNodeID: I490"@en-AU ;
    skos:definition "137  Manner of determining volumes of and fixing duty on beer"@en-AU ;
    skos:narrower C1901A00006:327 ;
    skos:prefLabel "Item I490"@en-AU ;
    dcat:accessURL "https://www.legislation.gov.au/C1901A00006/2024-07-01/2024-07-01/text/original/epub/OEBPS/document_2/document_2.html#_Toc172624245"^^xsd:anyURI .

C1901A00006:491 a legcons:Item,
        skos:Concept,
        dcat:Resource ;
    rdfs:label "Item I491"@en-AU ;
    rdfs:comment "142  Measurement for duty - GraphNodeID: I491"@en-AU ;
    skos:definition "142  Measurement for duty"@en-AU ;
    skos:narrower C1901A00006:327 ;
    skos:prefLabel "Item I491"@en-AU ;
    dcat:accessURL "https://www.legislation.gov.au/C1901A00006/2024-07-01/2024-07-01/text/original/epub/OEBPS/document_2/document_2.html#_Toc172624246"^^xsd:anyURI .

C1901A00006:492 a legcons:Item,
        skos:Concept,
        dcat:Resource ;
    rdfs:label "Item I492"@en-AU ;
    rdfs:comment "145  Value of goods sold - GraphNodeID: I492"@en-AU ;
    skos:definition "145  Value of goods sold"@en-AU ;
    skos:narrower C1901A00006:327 ;
    skos:prefLabel "Item I492"@en-AU ;
    dcat:accessURL "https://www.legislation.gov.au/C1901A00006/2024-07-01/2024-07-01/text/original/epub/OEBPS/document_2/document_2.html#_Toc172624247"^^xsd:anyURI .

C1901A00006:493 a legcons:Item,
        skos:Concept,
        dcat:Resource ;
    rdfs:label "Item I493"@en-AU ;
    rdfs:comment "148  Derelict goods dutiable - GraphNodeID: I493"@en-AU ;
    skos:definition "148  Derelict goods dutiable"@en-AU ;
    skos:narrower C1901A00006:327 ;
    skos:prefLabel "Item I493"@en-AU ;
    dcat:accessURL "https://www.legislation.gov.au/C1901A00006/2024-07-01/2024-07-01/text/original/epub/OEBPS/document_2/document_2.html#_Toc172624248"^^xsd:anyURI .

C1901A00006:494 a legcons:Item,
        skos:Concept,
        dcat:Resource ;
    rdfs:label "Item I494"@en-AU ;
    rdfs:comment "149  Duty on goods in report of cargo that are not produced or landed - GraphNodeID: I494"@en-AU ;
    skos:definition "149  Duty on goods in report of cargo that are not produced or landed"@en-AU ;
    skos:narrower C1901A00006:327 ;
    skos:prefLabel "Item I494"@en-AU ;
    dcat:accessURL "https://www.legislation.gov.au/C1901A00006/2024-07-01/2024-07-01/text/original/epub/OEBPS/document_2/document_2.html#_Toc172624249"^^xsd:anyURI .

C1901A00006:495 a legcons:Item,
        skos:Concept,
        dcat:Resource ;
    rdfs:label "Item I495"@en-AU ;
    rdfs:comment "150  Samples - GraphNodeID: I495"@en-AU ;
    skos:definition "150  Samples"@en-AU ;
    skos:narrower C1901A00006:327 ;
    skos:prefLabel "Item I495"@en-AU ;
    dcat:accessURL "https://www.legislation.gov.au/C1901A00006/2024-07-01/2024-07-01/text/original/epub/OEBPS/document_2/document_2.html#_Toc172624250"^^xsd:anyURI .

C1901A00006:496 a legcons:Item,
        skos:Concept,
        dcat:Resource ;
    rdfs:label "Item I496"@en-AU ;
    rdfs:comment "152  Alterations to agreements where duty altered - GraphNodeID: I496"@en-AU ;
    skos:definition "152  Alterations to agreements where duty altered"@en-AU ;
    skos:narrower C1901A00006:327 ;
    skos:prefLabel "Item I496"@en-AU ;
    dcat:accessURL "https://www.legislation.gov.au/C1901A00006/2024-07-01/2024-07-01/text/original/epub/OEBPS/document_2/document_2.html#_Toc172624251"^^xsd:anyURI .

C1901A00006:497 a legcons:Division,
        skos:Concept,
        dcat:Resource ;
    rdfs:label "Division D497"@en-AU ;
    rdfs:comment "Division 1 AACalculation of duty on certain alcoholic beverages - GraphNodeID: D497"@en-AU ;
    skos:definition "Division 1 AACalculation of duty on certain alcoholic beverages"@en-AU ;
    skos:narrower C1901A00006:475 ;
    skos:prefLabel "Division D497"@en-AU ;
    dcat:accessURL "https://www.legislation.gov.au/C1901A00006/2024-07-01/2024-07-01/text/original/epub/OEBPS/document_2/document_2.html#_Toc172624252"^^xsd:anyURI .

C1901A00006:498 a legcons:Item,
        skos:Concept,
        dcat:Resource ;
    rdfs:label "Item I498"@en-AU ;
    rdfs:comment "153 AA  Meaning of alcoholic beverage - GraphNodeID: I498"@en-AU ;
    skos:definition "153 AA  Meaning of alcoholic beverage"@en-AU ;
    skos:narrower C1901A00006:327 ;
    skos:prefLabel "Item I498"@en-AU ;
    dcat:accessURL "https://www.legislation.gov.au/C1901A00006/2024-07-01/2024-07-01/text/original/epub/OEBPS/document_2/document_2.html#_Toc172624253"^^xsd:anyURI .

C1901A00006:499 a legcons:Item,
        skos:Concept,
        dcat:Resource ;
    rdfs:label "Item I499"@en-AU ;
    rdfs:comment "153 AB  Customs duty to be paid according to labelled alcoholic strength of prescribed alcoholic beverages - GraphNodeID: I499"@en-AU ;
    skos:definition "153 AB  Customs duty to be paid according to labelled alcoholic strength of prescribed alcoholic beverages"@en-AU ;
    skos:narrower C1901A00006:327 ;
    skos:prefLabel "Item I499"@en-AU ;
    dcat:accessURL "https://www.legislation.gov.au/C1901A00006/2024-07-01/2024-07-01/text/original/epub/OEBPS/document_2/document_2.html#_Toc172624254"^^xsd:anyURI .

C1901A00006:5 a legcons:Item,
        skos:Concept,
        dcat:Resource ;
    rdfs:label "Item I5"@en-AU ;
    rdfs:comment "4  Definitions - GraphNodeID: I5"@en-AU ;
    skos:definition "4  Definitions"@en-AU ;
    skos:narrower C1901A00006:2 ;
    skos:prefLabel "Item I5"@en-AU ;
    dcat:accessURL "https://www.legislation.gov.au/C1901A00006/2024-07-01/2024-07-01/text/original/epub/OEBPS/document_1/document_1.html#_Toc172622979"^^xsd:anyURI .

C1901A00006:50 a legcons:Item,
        skos:Concept,
        dcat:Resource ;
    rdfs:label "Item I50"@en-AU ;
    rdfs:comment "45  Cancellation of securities - GraphNodeID: I50"@en-AU ;
    skos:definition "45  Cancellation of securities"@en-AU ;
    skos:narrower C1901A00006:33 ;
    skos:prefLabel "Item I50"@en-AU ;
    dcat:accessURL "https://www.legislation.gov.au/C1901A00006/2024-07-01/2024-07-01/text/original/epub/OEBPS/document_1/document_1.html#_Toc172623024"^^xsd:anyURI .

C1901A00006:500 a legcons:Item,
        skos:Concept,
        dcat:Resource ;
    rdfs:label "Item I500"@en-AU ;
    rdfs:comment "153 AC  Rules for working out strength of prescribed alcoholic beverages - GraphNodeID: I500"@en-AU ;
    skos:definition "153 AC  Rules for working out strength of prescribed alcoholic beverages"@en-AU ;
    skos:narrower C1901A00006:327 ;
    skos:prefLabel "Item I500"@en-AU ;
    dcat:accessURL "https://www.legislation.gov.au/C1901A00006/2024-07-01/2024-07-01/text/original/epub/OEBPS/document_2/document_2.html#_Toc172624255"^^xsd:anyURI .

C1901A00006:501 a legcons:Item,
        skos:Concept,
        dcat:Resource ;
    rdfs:label "Item I501"@en-AU ;
    rdfs:comment "153 AD  Obscuration - GraphNodeID: I501"@en-AU ;
    skos:definition "153 AD  Obscuration"@en-AU ;
    skos:narrower C1901A00006:327 ;
    skos:prefLabel "Item I501"@en-AU ;
    dcat:accessURL "https://www.legislation.gov.au/C1901A00006/2024-07-01/2024-07-01/text/original/epub/OEBPS/document_2/document_2.html#_Toc172624256"^^xsd:anyURI .

C1901A00006:502 a legcons:Division,
        skos:Concept,
        dcat:Resource ;
    rdfs:label "Division D502"@en-AU ;
    rdfs:comment "Division 1 ARules of origin of preference claim goods - GraphNodeID: D502"@en-AU ;
    skos:definition "Division 1 ARules of origin of preference claim goods"@en-AU ;
    skos:narrower C1901A00006:475 ;
    skos:prefLabel "Division D502"@en-AU ;
    dcat:accessURL "https://www.legislation.gov.au/C1901A00006/2024-07-01/2024-07-01/text/original/epub/OEBPS/document_2/document_2.html#_Toc172624257"^^xsd:anyURI .

C1901A00006:503 a legcons:Item,
        skos:Concept,
        dcat:Resource ;
    rdfs:label "Item I503"@en-AU ;
    rdfs:comment "153 A  Purpose of Division - GraphNodeID: I503"@en-AU ;
    skos:definition "153 A  Purpose of Division"@en-AU ;
    skos:narrower C1901A00006:327 ;
    skos:prefLabel "Item I503"@en-AU ;
    dcat:accessURL "https://www.legislation.gov.au/C1901A00006/2024-07-01/2024-07-01/text/original/epub/OEBPS/document_2/document_2.html#_Toc172624258"^^xsd:anyURI .

C1901A00006:504 a legcons:Item,
        skos:Concept,
        dcat:Resource ;
    rdfs:label "Item I504"@en-AU ;
    rdfs:comment "153 B  Definitions - GraphNodeID: I504"@en-AU ;
    skos:definition "153 B  Definitions"@en-AU ;
    skos:narrower C1901A00006:327 ;
    skos:prefLabel "Item I504"@en-AU ;
    dcat:accessURL "https://www.legislation.gov.au/C1901A00006/2024-07-01/2024-07-01/text/original/epub/OEBPS/document_2/document_2.html#_Toc172624259"^^xsd:anyURI .

C1901A00006:505 a legcons:Item,
        skos:Concept,
        dcat:Resource ;
    rdfs:label "Item I505"@en-AU ;
    rdfs:comment "153 C  Total expenditure of factory on materials - GraphNodeID: I505"@en-AU ;
    skos:definition "153 C  Total expenditure of factory on materials"@en-AU ;
    skos:narrower C1901A00006:327 ;
    skos:prefLabel "Item I505"@en-AU ;
    dcat:accessURL "https://www.legislation.gov.au/C1901A00006/2024-07-01/2024-07-01/text/original/epub/OEBPS/document_2/document_2.html#_Toc172624260"^^xsd:anyURI .

C1901A00006:506 a legcons:Item,
        skos:Concept,
        dcat:Resource ;
    rdfs:label "Item I506"@en-AU ;
    rdfs:comment "153 D  Allowable expenditure of factory on materials - GraphNodeID: I506"@en-AU ;
    skos:definition "153 D  Allowable expenditure of factory on materials"@en-AU ;
    skos:narrower C1901A00006:327 ;
    skos:prefLabel "Item I506"@en-AU ;
    dcat:accessURL "https://www.legislation.gov.au/C1901A00006/2024-07-01/2024-07-01/text/original/epub/OEBPS/document_2/document_2.html#_Toc172624261"^^xsd:anyURI .

C1901A00006:507 a legcons:Item,
        skos:Concept,
        dcat:Resource ;
    rdfs:label "Item I507"@en-AU ;
    rdfs:comment "153 E  Calculation of the cost of materials received at a factory - GraphNodeID: I507"@en-AU ;
    skos:definition "153 E  Calculation of the cost of materials received at a factory"@en-AU ;
    skos:narrower C1901A00006:327 ;
    skos:prefLabel "Item I507"@en-AU ;
    dcat:accessURL "https://www.legislation.gov.au/C1901A00006/2024-07-01/2024-07-01/text/original/epub/OEBPS/document_2/document_2.html#_Toc172624262"^^xsd:anyURI .

C1901A00006:508 a legcons:Item,
        skos:Concept,
        dcat:Resource ;
    rdfs:label "Item I508"@en-AU ;
    rdfs:comment "153 F  Allowable expenditure of factory on labour - GraphNodeID: I508"@en-AU ;
    skos:definition "153 F  Allowable expenditure of factory on labour"@en-AU ;
    skos:narrower C1901A00006:327 ;
    skos:prefLabel "Item I508"@en-AU ;
    dcat:accessURL "https://www.legislation.gov.au/C1901A00006/2024-07-01/2024-07-01/text/original/epub/OEBPS/document_2/document_2.html#_Toc172624263"^^xsd:anyURI .

C1901A00006:509 a legcons:Item,
        skos:Concept,
        dcat:Resource ;
    rdfs:label "Item I509"@en-AU ;
    rdfs:comment "153 G  Allowable expenditure of factory on overheads - GraphNodeID: I509"@en-AU ;
    skos:definition "153 G  Allowable expenditure of factory on overheads"@en-AU ;
    skos:narrower C1901A00006:327 ;
    skos:prefLabel "Item I509"@en-AU ;
    dcat:accessURL "https://www.legislation.gov.au/C1901A00006/2024-07-01/2024-07-01/text/original/epub/OEBPS/document_2/document_2.html#_Toc172624264"^^xsd:anyURI .

C1901A00006:51 a legcons:Item,
        skos:Concept,
        dcat:Resource ;
    rdfs:label "Item I51"@en-AU ;
    rdfs:comment "46  New securities - GraphNodeID: I51"@en-AU ;
    skos:definition "46  New securities"@en-AU ;
    skos:narrower C1901A00006:33 ;
    skos:prefLabel "Item I51"@en-AU ;
    dcat:accessURL "https://www.legislation.gov.au/C1901A00006/2024-07-01/2024-07-01/text/original/epub/OEBPS/document_1/document_1.html#_Toc172623025"^^xsd:anyURI .

C1901A00006:510 a legcons:Item,
        skos:Concept,
        dcat:Resource ;
    rdfs:label "Item I510"@en-AU ;
    rdfs:comment "153 H  Unmanufactured goods - GraphNodeID: I510"@en-AU ;
    skos:definition "153 H  Unmanufactured goods"@en-AU ;
    skos:narrower C1901A00006:327 ;
    skos:prefLabel "Item I510"@en-AU ;
    dcat:accessURL "https://www.legislation.gov.au/C1901A00006/2024-07-01/2024-07-01/text/original/epub/OEBPS/document_2/document_2.html#_Toc172624265"^^xsd:anyURI .

C1901A00006:511 a legcons:Item,
        skos:Concept,
        dcat:Resource ;
    rdfs:label "Item I511"@en-AU ;
    rdfs:comment "153 L  Manufactured goods originating in Papua New Guinea or a Forum Island Country - GraphNodeID: I511"@en-AU ;
    skos:definition "153 L  Manufactured goods originating in Papua New Guinea or a Forum Island Country"@en-AU ;
    skos:narrower C1901A00006:327 ;
    skos:prefLabel "Item I511"@en-AU ;
    dcat:accessURL "https://www.legislation.gov.au/C1901A00006/2024-07-01/2024-07-01/text/original/epub/OEBPS/document_2/document_2.html#_Toc172624266"^^xsd:anyURI .

C1901A00006:512 a legcons:Item,
        skos:Concept,
        dcat:Resource ;
    rdfs:label "Item I512"@en-AU ;
    rdfs:comment "153 LA  Modification of section 153 L in special circumstances - GraphNodeID: I512"@en-AU ;
    skos:definition "153 LA  Modification of section 153 L in special circumstances"@en-AU ;
    skos:narrower C1901A00006:327 ;
    skos:prefLabel "Item I512"@en-AU ;
    dcat:accessURL "https://www.legislation.gov.au/C1901A00006/2024-07-01/2024-07-01/text/original/epub/OEBPS/document_2/document_2.html#_Toc172624267"^^xsd:anyURI .

C1901A00006:513 a legcons:Item,
        skos:Concept,
        dcat:Resource ;
    rdfs:label "Item I513"@en-AU ;
    rdfs:comment "153 M  Manufactured goods originating in a particular Developing Country - GraphNodeID: I513"@en-AU ;
    skos:definition "153 M  Manufactured goods originating in a particular Developing Country"@en-AU ;
    skos:narrower C1901A00006:327 ;
    skos:prefLabel "Item I513"@en-AU ;
    dcat:accessURL "https://www.legislation.gov.au/C1901A00006/2024-07-01/2024-07-01/text/original/epub/OEBPS/document_2/document_2.html#_Toc172624268"^^xsd:anyURI .

C1901A00006:514 a legcons:Item,
        skos:Concept,
        dcat:Resource ;
    rdfs:label "Item I514"@en-AU ;
    rdfs:comment "153 N  Manufactured goods originating in a Developing Country but not in any particular Developing Country - GraphNodeID: I514"@en-AU ;
    skos:definition "153 N  Manufactured goods originating in a Developing Country but not in any particular Developing Country"@en-AU ;
    skos:narrower C1901A00006:327 ;
    skos:prefLabel "Item I514"@en-AU ;
    dcat:accessURL "https://www.legislation.gov.au/C1901A00006/2024-07-01/2024-07-01/text/original/epub/OEBPS/document_2/document_2.html#_Toc172624269"^^xsd:anyURI .

C1901A00006:515 a legcons:Item,
        skos:Concept,
        dcat:Resource ;
    rdfs:label "Item I515"@en-AU ;
    rdfs:comment "153 NA  Manufactured goods originating in a Least Developed Country - GraphNodeID: I515"@en-AU ;
    skos:definition "153 NA  Manufactured goods originating in a Least Developed Country"@en-AU ;
    skos:narrower C1901A00006:327 ;
    skos:prefLabel "Item I515"@en-AU ;
    dcat:accessURL "https://www.legislation.gov.au/C1901A00006/2024-07-01/2024-07-01/text/original/epub/OEBPS/document_2/document_2.html#_Toc172624270"^^xsd:anyURI .

C1901A00006:516 a legcons:Item,
        skos:Concept,
        dcat:Resource ;
    rdfs:label "Item I516"@en-AU ;
    rdfs:comment "153 P  Manufactured goods originating in Canada - GraphNodeID: I516"@en-AU ;
    skos:definition "153 P  Manufactured goods originating in Canada"@en-AU ;
    skos:narrower C1901A00006:327 ;
    skos:prefLabel "Item I516"@en-AU ;
    dcat:accessURL "https://www.legislation.gov.au/C1901A00006/2024-07-01/2024-07-01/text/original/epub/OEBPS/document_2/document_2.html#_Toc172624271"^^xsd:anyURI .

C1901A00006:517 a legcons:Item,
        skos:Concept,
        dcat:Resource ;
    rdfs:label "Item I517"@en-AU ;
    rdfs:comment "153 Q  Manufactured goods originating in a country that is not a preference country - GraphNodeID: I517"@en-AU ;
    skos:definition "153 Q  Manufactured goods originating in a country that is not a preference country"@en-AU ;
    skos:narrower C1901A00006:327 ;
    skos:prefLabel "Item I517"@en-AU ;
    dcat:accessURL "https://www.legislation.gov.au/C1901A00006/2024-07-01/2024-07-01/text/original/epub/OEBPS/document_2/document_2.html#_Toc172624272"^^xsd:anyURI .

C1901A00006:518 a legcons:Item,
        skos:Concept,
        dcat:Resource ;
    rdfs:label "Item I518"@en-AU ;
    rdfs:comment "153 R  Are goods commercially manufactured in Australia - GraphNodeID: I518"@en-AU ;
    skos:definition "153 R  Are goods commercially manufactured in Australia"@en-AU ;
    skos:narrower C1901A00006:327 ;
    skos:prefLabel "Item I518"@en-AU ;
    dcat:accessURL "https://www.legislation.gov.au/C1901A00006/2024-07-01/2024-07-01/text/original/epub/OEBPS/document_2/document_2.html#_Toc172624273"^^xsd:anyURI .

C1901A00006:519 a legcons:Item,
        skos:Concept,
        dcat:Resource ;
    rdfs:label "Item I519"@en-AU ;
    rdfs:comment "153 S  Rule against double counting - GraphNodeID: I519"@en-AU ;
    skos:definition "153 S  Rule against double counting"@en-AU ;
    skos:narrower C1901A00006:327 ;
    skos:prefLabel "Item I519"@en-AU ;
    dcat:accessURL "https://www.legislation.gov.au/C1901A00006/2024-07-01/2024-07-01/text/original/epub/OEBPS/document_2/document_2.html#_Toc172624274"^^xsd:anyURI .

C1901A00006:52 a legcons:Item,
        skos:Concept,
        dcat:Resource ;
    rdfs:label "Item I52"@en-AU ;
    rdfs:comment "47  Form of security - GraphNodeID: I52"@en-AU ;
    skos:definition "47  Form of security"@en-AU ;
    skos:narrower C1901A00006:33 ;
    skos:prefLabel "Item I52"@en-AU ;
    dcat:accessURL "https://www.legislation.gov.au/C1901A00006/2024-07-01/2024-07-01/text/original/epub/OEBPS/document_1/document_1.html#_Toc172623026"^^xsd:anyURI .

C1901A00006:522 a legcons:Item,
        skos:Concept,
        dcat:Resource ;
    rdfs:label "Item I522"@en-AU ;
    rdfs:comment "153 XC  Simplified outline of this Division - GraphNodeID: I522"@en-AU ;
    skos:definition "153 XC  Simplified outline of this Division"@en-AU ;
    skos:narrower C1901A00006:521 ;
    skos:prefLabel "Item I522"@en-AU ;
    dcat:accessURL "https://www.legislation.gov.au/C1901A00006/2024-07-01/2024-07-01/text/original/epub/OEBPS/document_2/document_2.html#_Toc172624277"^^xsd:anyURI .

C1901A00006:523 a legcons:Item,
        skos:Concept,
        dcat:Resource ;
    rdfs:label "Item I523"@en-AU ;
    rdfs:comment "153 XD  Interpretation - GraphNodeID: I523"@en-AU ;
    skos:definition "153 XD  Interpretation"@en-AU ;
    skos:narrower C1901A00006:521 ;
    skos:prefLabel "Item I523"@en-AU ;
    dcat:accessURL "https://www.legislation.gov.au/C1901A00006/2024-07-01/2024-07-01/text/original/epub/OEBPS/document_2/document_2.html#_Toc172624278"^^xsd:anyURI .

C1901A00006:525 a legcons:Item,
        skos:Concept,
        dcat:Resource ;
    rdfs:label "Item I525"@en-AU ;
    rdfs:comment "153 XE  Goods wholly obtained or produced entirely in Singapore or in Singapore and Australia - GraphNodeID: I525"@en-AU ;
    skos:definition "153 XE  Goods wholly obtained or produced entirely in Singapore or in Singapore and Australia"@en-AU ;
    skos:narrower C1901A00006:524 ;
    skos:prefLabel "Item I525"@en-AU ;
    dcat:accessURL "https://www.legislation.gov.au/C1901A00006/2024-07-01/2024-07-01/text/original/epub/OEBPS/document_2/document_2.html#_Toc172624280"^^xsd:anyURI .

C1901A00006:527 a legcons:Item,
        skos:Concept,
        dcat:Resource ;
    rdfs:label "Item I527"@en-AU ;
    rdfs:comment "153 XF  Goods produced in Singapore or in Singapore and Australia from originating materials - GraphNodeID: I527"@en-AU ;
    skos:definition "153 XF  Goods produced in Singapore or in Singapore and Australia from originating materials"@en-AU ;
    skos:narrower C1901A00006:526 ;
    skos:prefLabel "Item I527"@en-AU ;
    dcat:accessURL "https://www.legislation.gov.au/C1901A00006/2024-07-01/2024-07-01/text/original/epub/OEBPS/document_2/document_2.html#_Toc172624282"^^xsd:anyURI .

C1901A00006:529 a legcons:Item,
        skos:Concept,
        dcat:Resource ;
    rdfs:label "Item I529"@en-AU ;
    rdfs:comment "153 XG  Goods produced in Singapore or in Singapore and Australia from non originating materials - GraphNodeID: I529"@en-AU ;
    skos:definition "153 XG  Goods produced in Singapore or in Singapore and Australia from non originating materials"@en-AU ;
    skos:narrower C1901A00006:528 ;
    skos:prefLabel "Item I529"@en-AU ;
    dcat:accessURL "https://www.legislation.gov.au/C1901A00006/2024-07-01/2024-07-01/text/original/epub/OEBPS/document_2/document_2.html#_Toc172624284"^^xsd:anyURI .

C1901A00006:53 a legcons:Item,
        skos:Concept,
        dcat:Resource ;
    rdfs:label "Item I53"@en-AU ;
    rdfs:comment "48  Effect of security - GraphNodeID: I53"@en-AU ;
    skos:definition "48  Effect of security"@en-AU ;
    skos:narrower C1901A00006:33 ;
    skos:prefLabel "Item I53"@en-AU ;
    dcat:accessURL "https://www.legislation.gov.au/C1901A00006/2024-07-01/2024-07-01/text/original/epub/OEBPS/document_1/document_1.html#_Toc172623027"^^xsd:anyURI .

C1901A00006:530 a legcons:Item,
        skos:Concept,
        dcat:Resource ;
    rdfs:label "Item I530"@en-AU ;
    rdfs:comment "153 XH  Packaging materials and containers - GraphNodeID: I530"@en-AU ;
    skos:definition "153 XH  Packaging materials and containers"@en-AU ;
    skos:narrower C1901A00006:528 ;
    skos:prefLabel "Item I530"@en-AU ;
    dcat:accessURL "https://www.legislation.gov.au/C1901A00006/2024-07-01/2024-07-01/text/original/epub/OEBPS/document_2/document_2.html#_Toc172624285"^^xsd:anyURI .

C1901A00006:532 a legcons:Item,
        skos:Concept,
        dcat:Resource ;
    rdfs:label "Item I532"@en-AU ;
    rdfs:comment "153 XI  Goods that are accessories spare parts tools or instructional or other information materials - GraphNodeID: I532"@en-AU ;
    skos:definition "153 XI  Goods that are accessories spare parts tools or instructional or other information materials"@en-AU ;
    skos:narrower C1901A00006:531 ;
    skos:prefLabel "Item I532"@en-AU ;
    dcat:accessURL "https://www.legislation.gov.au/C1901A00006/2024-07-01/2024-07-01/text/original/epub/OEBPS/document_2/document_2.html#_Toc172624287"^^xsd:anyURI .

C1901A00006:534 a legcons:Item,
        skos:Concept,
        dcat:Resource ;
    rdfs:label "Item I534"@en-AU ;
    rdfs:comment "153 XJ  Consignment - GraphNodeID: I534"@en-AU ;
    skos:definition "153 XJ  Consignment"@en-AU ;
    skos:narrower C1901A00006:533 ;
    skos:prefLabel "Item I534"@en-AU ;
    dcat:accessURL "https://www.legislation.gov.au/C1901A00006/2024-07-01/2024-07-01/text/original/epub/OEBPS/document_2/document_2.html#_Toc172624289"^^xsd:anyURI .

C1901A00006:536 a legcons:Item,
        skos:Concept,
        dcat:Resource ;
    rdfs:label "Item I536"@en-AU ;
    rdfs:comment "153 XK  Regulations - GraphNodeID: I536"@en-AU ;
    skos:definition "153 XK  Regulations"@en-AU ;
    skos:narrower C1901A00006:535 ;
    skos:prefLabel "Item I536"@en-AU ;
    dcat:accessURL "https://www.legislation.gov.au/C1901A00006/2024-07-01/2024-07-01/text/original/epub/OEBPS/document_2/document_2.html#_Toc172624291"^^xsd:anyURI .

C1901A00006:539 a legcons:Item,
        skos:Concept,
        dcat:Resource ;
    rdfs:label "Item I539"@en-AU ;
    rdfs:comment "153 Y  Simplified outline - GraphNodeID: I539"@en-AU ;
    skos:definition "153 Y  Simplified outline"@en-AU ;
    skos:narrower C1901A00006:538 ;
    skos:prefLabel "Item I539"@en-AU ;
    dcat:accessURL "https://www.legislation.gov.au/C1901A00006/2024-07-01/2024-07-01/text/original/epub/OEBPS/document_2/document_2.html#_Toc172624294"^^xsd:anyURI .

C1901A00006:540 a legcons:Item,
        skos:Concept,
        dcat:Resource ;
    rdfs:label "Item I540"@en-AU ;
    rdfs:comment "153 YA  Interpretation - GraphNodeID: I540"@en-AU ;
    skos:definition "153 YA  Interpretation"@en-AU ;
    skos:narrower C1901A00006:538 ;
    skos:prefLabel "Item I540"@en-AU ;
    dcat:accessURL "https://www.legislation.gov.au/C1901A00006/2024-07-01/2024-07-01/text/original/epub/OEBPS/document_2/document_2.html#_Toc172624295"^^xsd:anyURI .

C1901A00006:542 a legcons:Item,
        skos:Concept,
        dcat:Resource ;
    rdfs:label "Item I542"@en-AU ;
    rdfs:comment "153 YB  Goods wholly obtained or produced entirely in the US - GraphNodeID: I542"@en-AU ;
    skos:definition "153 YB  Goods wholly obtained or produced entirely in the US"@en-AU ;
    skos:narrower C1901A00006:541 ;
    skos:prefLabel "Item I542"@en-AU ;
    dcat:accessURL "https://www.legislation.gov.au/C1901A00006/2024-07-01/2024-07-01/text/original/epub/OEBPS/document_2/document_2.html#_Toc172624297"^^xsd:anyURI .

C1901A00006:544 a legcons:Item,
        skos:Concept,
        dcat:Resource ;
    rdfs:label "Item I544"@en-AU ;
    rdfs:comment "153 YC  Goods produced entirely in the US or in the US and Australia exclusively from originating materials - GraphNodeID: I544"@en-AU ;
    skos:definition "153 YC  Goods produced entirely in the US or in the US and Australia exclusively from originating materials"@en-AU ;
    skos:narrower C1901A00006:543 ;
    skos:prefLabel "Item I544"@en-AU ;
    dcat:accessURL "https://www.legislation.gov.au/C1901A00006/2024-07-01/2024-07-01/text/original/epub/OEBPS/document_2/document_2.html#_Toc172624299"^^xsd:anyURI .

C1901A00006:546 a legcons:Item,
        skos:Concept,
        dcat:Resource ;
    rdfs:label "Item I546"@en-AU ;
    rdfs:comment "153 YD  Goods produced in the US or in the US and Australia from non originating materials - GraphNodeID: I546"@en-AU ;
    skos:definition "153 YD  Goods produced in the US or in the US and Australia from non originating materials"@en-AU ;
    skos:narrower C1901A00006:545 ;
    skos:prefLabel "Item I546"@en-AU ;
    dcat:accessURL "https://www.legislation.gov.au/C1901A00006/2024-07-01/2024-07-01/text/original/epub/OEBPS/document_2/document_2.html#_Toc172624301"^^xsd:anyURI .

C1901A00006:548 a legcons:Item,
        skos:Concept,
        dcat:Resource ;
    rdfs:label "Item I548"@en-AU ;
    rdfs:comment "153 YJ  Goods that are standard accessories spare parts or tools - GraphNodeID: I548"@en-AU ;
    skos:definition "153 YJ  Goods that are standard accessories spare parts or tools"@en-AU ;
    skos:narrower C1901A00006:547 ;
    skos:prefLabel "Item I548"@en-AU ;
    dcat:accessURL "https://www.legislation.gov.au/C1901A00006/2024-07-01/2024-07-01/text/original/epub/OEBPS/document_2/document_2.html#_Toc172624303"^^xsd:anyURI .

C1901A00006:550 a legcons:Item,
        skos:Concept,
        dcat:Resource ;
    rdfs:label "Item I550"@en-AU ;
    rdfs:comment "153 YK  Packaging materials and containers - GraphNodeID: I550"@en-AU ;
    skos:definition "153 YK  Packaging materials and containers"@en-AU ;
    skos:narrower C1901A00006:549 ;
    skos:prefLabel "Item I550"@en-AU ;
    dcat:accessURL "https://www.legislation.gov.au/C1901A00006/2024-07-01/2024-07-01/text/original/epub/OEBPS/document_2/document_2.html#_Toc172624305"^^xsd:anyURI .

C1901A00006:552 a legcons:Item,
        skos:Concept,
        dcat:Resource ;
    rdfs:label "Item I552"@en-AU ;
    rdfs:comment "153 YL  Consignment - GraphNodeID: I552"@en-AU ;
    skos:definition "153 YL  Consignment"@en-AU ;
    skos:narrower C1901A00006:551 ;
    skos:prefLabel "Item I552"@en-AU ;
    dcat:accessURL "https://www.legislation.gov.au/C1901A00006/2024-07-01/2024-07-01/text/original/epub/OEBPS/document_2/document_2.html#_Toc172624307"^^xsd:anyURI .

C1901A00006:554 a legcons:Item,
        skos:Concept,
        dcat:Resource ;
    rdfs:label "Item I554"@en-AU ;
    rdfs:comment "153 YM  Regulations - GraphNodeID: I554"@en-AU ;
    skos:definition "153 YM  Regulations"@en-AU ;
    skos:narrower C1901A00006:553 ;
    skos:prefLabel "Item I554"@en-AU ;
    dcat:accessURL "https://www.legislation.gov.au/C1901A00006/2024-07-01/2024-07-01/text/original/epub/OEBPS/document_2/document_2.html#_Toc172624309"^^xsd:anyURI .

C1901A00006:557 a legcons:Item,
        skos:Concept,
        dcat:Resource ;
    rdfs:label "Item I557"@en-AU ;
    rdfs:comment "153 Z  Simplified outline - GraphNodeID: I557"@en-AU ;
    skos:definition "153 Z  Simplified outline"@en-AU ;
    skos:narrower C1901A00006:556 ;
    skos:prefLabel "Item I557"@en-AU ;
    dcat:accessURL "https://www.legislation.gov.au/C1901A00006/2024-07-01/2024-07-01/text/original/epub/OEBPS/document_2/document_2.html#_Toc172624312"^^xsd:anyURI .

C1901A00006:558 a legcons:Item,
        skos:Concept,
        dcat:Resource ;
    rdfs:label "Item I558"@en-AU ;
    rdfs:comment "153 ZA  Interpretation - GraphNodeID: I558"@en-AU ;
    skos:definition "153 ZA  Interpretation"@en-AU ;
    skos:narrower C1901A00006:556 ;
    skos:prefLabel "Item I558"@en-AU ;
    dcat:accessURL "https://www.legislation.gov.au/C1901A00006/2024-07-01/2024-07-01/text/original/epub/OEBPS/document_2/document_2.html#_Toc172624313"^^xsd:anyURI .

C1901A00006:56 a legcons:Item,
        skos:Concept,
        dcat:Resource ;
    rdfs:label "Item I56"@en-AU ;
    rdfs:comment "49  Importation - GraphNodeID: I56"@en-AU ;
    skos:definition "49  Importation"@en-AU ;
    skos:narrower C1901A00006:55 ;
    skos:prefLabel "Item I56"@en-AU ;
    dcat:accessURL "https://www.legislation.gov.au/C1901A00006/2024-07-01/2024-07-01/text/original/epub/OEBPS/document_1/document_1.html#_Toc172623030"^^xsd:anyURI .

C1901A00006:560 a legcons:Item,
        skos:Concept,
        dcat:Resource ;
    rdfs:label "Item I560"@en-AU ;
    rdfs:comment "153 ZB  Wholly obtained goods of Thailand - GraphNodeID: I560"@en-AU ;
    skos:definition "153 ZB  Wholly obtained goods of Thailand"@en-AU ;
    skos:narrower C1901A00006:559 ;
    skos:prefLabel "Item I560"@en-AU ;
    dcat:accessURL "https://www.legislation.gov.au/C1901A00006/2024-07-01/2024-07-01/text/original/epub/OEBPS/document_2/document_2.html#_Toc172624315"^^xsd:anyURI .

C1901A00006:562 a legcons:Item,
        skos:Concept,
        dcat:Resource ;
    rdfs:label "Item I562"@en-AU ;
    rdfs:comment "153 ZC  Goods produced entirely in Thailand or in Thailand and Australia - GraphNodeID: I562"@en-AU ;
    skos:definition "153 ZC  Goods produced entirely in Thailand or in Thailand and Australia"@en-AU ;
    skos:narrower C1901A00006:561 ;
    skos:prefLabel "Item I562"@en-AU ;
    dcat:accessURL "https://www.legislation.gov.au/C1901A00006/2024-07-01/2024-07-01/text/original/epub/OEBPS/document_2/document_2.html#_Toc172624317"^^xsd:anyURI .

C1901A00006:564 a legcons:Item,
        skos:Concept,
        dcat:Resource ;
    rdfs:label "Item I564"@en-AU ;
    rdfs:comment "153 ZF  Goods that are standard accessories spare parts or tools - GraphNodeID: I564"@en-AU ;
    skos:definition "153 ZF  Goods that are standard accessories spare parts or tools"@en-AU ;
    skos:narrower C1901A00006:563 ;
    skos:prefLabel "Item I564"@en-AU ;
    dcat:accessURL "https://www.legislation.gov.au/C1901A00006/2024-07-01/2024-07-01/text/original/epub/OEBPS/document_2/document_2.html#_Toc172624319"^^xsd:anyURI .

C1901A00006:566 a legcons:Item,
        skos:Concept,
        dcat:Resource ;
    rdfs:label "Item I566"@en-AU ;
    rdfs:comment "153 ZG  Packaging materials and containers - GraphNodeID: I566"@en-AU ;
    skos:definition "153 ZG  Packaging materials and containers"@en-AU ;
    skos:narrower C1901A00006:565 ;
    skos:prefLabel "Item I566"@en-AU ;
    dcat:accessURL "https://www.legislation.gov.au/C1901A00006/2024-07-01/2024-07-01/text/original/epub/OEBPS/document_2/document_2.html#_Toc172624321"^^xsd:anyURI .

C1901A00006:568 a legcons:Item,
        skos:Concept,
        dcat:Resource ;
    rdfs:label "Item I568"@en-AU ;
    rdfs:comment "153 ZH  Consignment - GraphNodeID: I568"@en-AU ;
    skos:definition "153 ZH  Consignment"@en-AU ;
    skos:narrower C1901A00006:567 ;
    skos:prefLabel "Item I568"@en-AU ;
    dcat:accessURL "https://www.legislation.gov.au/C1901A00006/2024-07-01/2024-07-01/text/original/epub/OEBPS/document_2/document_2.html#_Toc172624323"^^xsd:anyURI .

C1901A00006:57 a legcons:Item,
        skos:Concept,
        dcat:Resource ;
    rdfs:label "Item I57"@en-AU ;
    rdfs:comment "49 A  Ships and aircraft deemed to be imported - GraphNodeID: I57"@en-AU ;
    skos:definition "49 A  Ships and aircraft deemed to be imported"@en-AU ;
    skos:narrower C1901A00006:55 ;
    skos:prefLabel "Item I57"@en-AU ;
    dcat:accessURL "https://www.legislation.gov.au/C1901A00006/2024-07-01/2024-07-01/text/original/epub/OEBPS/document_1/document_1.html#_Toc172623031"^^xsd:anyURI .

C1901A00006:570 a legcons:Item,
        skos:Concept,
        dcat:Resource ;
    rdfs:label "Item I570"@en-AU ;
    rdfs:comment "153 ZI  Regulations - GraphNodeID: I570"@en-AU ;
    skos:definition "153 ZI  Regulations"@en-AU ;
    skos:narrower C1901A00006:569 ;
    skos:prefLabel "Item I570"@en-AU ;
    dcat:accessURL "https://www.legislation.gov.au/C1901A00006/2024-07-01/2024-07-01/text/original/epub/OEBPS/document_2/document_2.html#_Toc172624325"^^xsd:anyURI .

C1901A00006:573 a legcons:Item,
        skos:Concept,
        dcat:Resource ;
    rdfs:label "Item I573"@en-AU ;
    rdfs:comment "153 ZIA  Simplified outline - GraphNodeID: I573"@en-AU ;
    skos:definition "153 ZIA  Simplified outline"@en-AU ;
    skos:narrower C1901A00006:572 ;
    skos:prefLabel "Item I573"@en-AU ;
    dcat:accessURL "https://www.legislation.gov.au/C1901A00006/2024-07-01/2024-07-01/text/original/epub/OEBPS/document_2/document_2.html#_Toc172624328"^^xsd:anyURI .

C1901A00006:574 a legcons:Item,
        skos:Concept,
        dcat:Resource ;
    rdfs:label "Item I574"@en-AU ;
    rdfs:comment "153 ZIB  Interpretation - GraphNodeID: I574"@en-AU ;
    skos:definition "153 ZIB  Interpretation"@en-AU ;
    skos:narrower C1901A00006:572 ;
    skos:prefLabel "Item I574"@en-AU ;
    dcat:accessURL "https://www.legislation.gov.au/C1901A00006/2024-07-01/2024-07-01/text/original/epub/OEBPS/document_2/document_2.html#_Toc172624329"^^xsd:anyURI .

C1901A00006:576 a legcons:Item,
        skos:Concept,
        dcat:Resource ;
    rdfs:label "Item I576"@en-AU ;
    rdfs:comment "153 ZIC  Goods wholly obtained or produced in New Zealand or New Zealand and Australia - GraphNodeID: I576"@en-AU ;
    skos:definition "153 ZIC  Goods wholly obtained or produced in New Zealand or New Zealand and Australia"@en-AU ;
    skos:narrower C1901A00006:575 ;
    skos:prefLabel "Item I576"@en-AU ;
    dcat:accessURL "https://www.legislation.gov.au/C1901A00006/2024-07-01/2024-07-01/text/original/epub/OEBPS/document_2/document_2.html#_Toc172624331"^^xsd:anyURI .

C1901A00006:578 a legcons:Item,
        skos:Concept,
        dcat:Resource ;
    rdfs:label "Item I578"@en-AU ;
    rdfs:comment "153 ZID  Goods produced in New Zealand or New Zealand and Australia from originating materials - GraphNodeID: I578"@en-AU ;
    skos:definition "153 ZID  Goods produced in New Zealand or New Zealand and Australia from originating materials"@en-AU ;
    skos:narrower C1901A00006:577 ;
    skos:prefLabel "Item I578"@en-AU ;
    dcat:accessURL "https://www.legislation.gov.au/C1901A00006/2024-07-01/2024-07-01/text/original/epub/OEBPS/document_2/document_2.html#_Toc172624333"^^xsd:anyURI .

C1901A00006:58 a legcons:Item,
        skos:Concept,
        dcat:Resource ;
    rdfs:label "Item I58"@en-AU ;
    rdfs:comment "49 B  Installations and goods deemed to be imported - GraphNodeID: I58"@en-AU ;
    skos:definition "49 B  Installations and goods deemed to be imported"@en-AU ;
    skos:narrower C1901A00006:55 ;
    skos:prefLabel "Item I58"@en-AU ;
    dcat:accessURL "https://www.legislation.gov.au/C1901A00006/2024-07-01/2024-07-01/text/original/epub/OEBPS/document_1/document_1.html#_Toc172623032"^^xsd:anyURI .

C1901A00006:580 a legcons:Item,
        skos:Concept,
        dcat:Resource ;
    rdfs:label "Item I580"@en-AU ;
    rdfs:comment "153 ZIE  Goods produced in New Zealand or New Zealand and Australia from non originating materials - GraphNodeID: I580"@en-AU ;
    skos:definition "153 ZIE  Goods produced in New Zealand or New Zealand and Australia from non originating materials"@en-AU ;
    skos:narrower C1901A00006:579 ;
    skos:prefLabel "Item I580"@en-AU ;
    dcat:accessURL "https://www.legislation.gov.au/C1901A00006/2024-07-01/2024-07-01/text/original/epub/OEBPS/document_2/document_2.html#_Toc172624335"^^xsd:anyURI .

C1901A00006:581 a legcons:Item,
        skos:Concept,
        dcat:Resource ;
    rdfs:label "Item I581"@en-AU ;
    rdfs:comment "153 ZIF  Packaging materials and containers - GraphNodeID: I581"@en-AU ;
    skos:definition "153 ZIF  Packaging materials and containers"@en-AU ;
    skos:narrower C1901A00006:579 ;
    skos:prefLabel "Item I581"@en-AU ;
    dcat:accessURL "https://www.legislation.gov.au/C1901A00006/2024-07-01/2024-07-01/text/original/epub/OEBPS/document_2/document_2.html#_Toc172624336"^^xsd:anyURI .

C1901A00006:583 a legcons:Item,
        skos:Concept,
        dcat:Resource ;
    rdfs:label "Item I583"@en-AU ;
    rdfs:comment "153 ZIG  Goods that are standard accessories spare parts or tools - GraphNodeID: I583"@en-AU ;
    skos:definition "153 ZIG  Goods that are standard accessories spare parts or tools"@en-AU ;
    skos:narrower C1901A00006:582 ;
    skos:prefLabel "Item I583"@en-AU ;
    dcat:accessURL "https://www.legislation.gov.au/C1901A00006/2024-07-01/2024-07-01/text/original/epub/OEBPS/document_2/document_2.html#_Toc172624338"^^xsd:anyURI .

C1901A00006:585 a legcons:Item,
        skos:Concept,
        dcat:Resource ;
    rdfs:label "Item I585"@en-AU ;
    rdfs:comment "153 ZIH  Goods wholly manufactured in New Zealand - GraphNodeID: I585"@en-AU ;
    skos:definition "153 ZIH  Goods wholly manufactured in New Zealand"@en-AU ;
    skos:narrower C1901A00006:584 ;
    skos:prefLabel "Item I585"@en-AU ;
    dcat:accessURL "https://www.legislation.gov.au/C1901A00006/2024-07-01/2024-07-01/text/original/epub/OEBPS/document_2/document_2.html#_Toc172624340"^^xsd:anyURI .

C1901A00006:587 a legcons:Item,
        skos:Concept,
        dcat:Resource ;
    rdfs:label "Item I587"@en-AU ;
    rdfs:comment "153 ZIJ  Non qualifying operations - GraphNodeID: I587"@en-AU ;
    skos:definition "153 ZIJ  Non qualifying operations"@en-AU ;
    skos:narrower C1901A00006:586 ;
    skos:prefLabel "Item I587"@en-AU ;
    dcat:accessURL "https://www.legislation.gov.au/C1901A00006/2024-07-01/2024-07-01/text/original/epub/OEBPS/document_2/document_2.html#_Toc172624342"^^xsd:anyURI .

C1901A00006:589 a legcons:Item,
        skos:Concept,
        dcat:Resource ;
    rdfs:label "Item I589"@en-AU ;
    rdfs:comment "153 ZIK  Consignment - GraphNodeID: I589"@en-AU ;
    skos:definition "153 ZIK  Consignment"@en-AU ;
    skos:narrower C1901A00006:588 ;
    skos:prefLabel "Item I589"@en-AU ;
    dcat:accessURL "https://www.legislation.gov.au/C1901A00006/2024-07-01/2024-07-01/text/original/epub/OEBPS/document_2/document_2.html#_Toc172624344"^^xsd:anyURI .

C1901A00006:59 a legcons:Item,
        skos:Concept,
        dcat:Resource ;
    rdfs:label "Item I59"@en-AU ;
    rdfs:comment "49 C  Obligations under this Part may be satisfied in accordance with a trusted trader agreement - GraphNodeID: I59"@en-AU ;
    skos:definition "49 C  Obligations under this Part may be satisfied in accordance with a trusted trader agreement"@en-AU ;
    skos:narrower C1901A00006:55 ;
    skos:prefLabel "Item I59"@en-AU ;
    dcat:accessURL "https://www.legislation.gov.au/C1901A00006/2024-07-01/2024-07-01/text/original/epub/OEBPS/document_1/document_1.html#_Toc172623033"^^xsd:anyURI .

C1901A00006:591 a legcons:Item,
        skos:Concept,
        dcat:Resource ;
    rdfs:label "Item I591"@en-AU ;
    rdfs:comment "153 ZIKA  Regulations - GraphNodeID: I591"@en-AU ;
    skos:definition "153 ZIKA  Regulations"@en-AU ;
    skos:narrower C1901A00006:590 ;
    skos:prefLabel "Item I591"@en-AU ;
    dcat:accessURL "https://www.legislation.gov.au/C1901A00006/2024-07-01/2024-07-01/text/original/epub/OEBPS/document_2/document_2.html#_Toc172624346"^^xsd:anyURI .

C1901A00006:594 a legcons:Item,
        skos:Concept,
        dcat:Resource ;
    rdfs:label "Item I594"@en-AU ;
    rdfs:comment "153 ZIL  Simplified outline of this Division - GraphNodeID: I594"@en-AU ;
    skos:definition "153 ZIL  Simplified outline of this Division"@en-AU ;
    skos:narrower C1901A00006:593 ;
    skos:prefLabel "Item I594"@en-AU ;
    dcat:accessURL "https://www.legislation.gov.au/C1901A00006/2024-07-01/2024-07-01/text/original/epub/OEBPS/document_2/document_2.html#_Toc172624349"^^xsd:anyURI .

C1901A00006:595 a legcons:Item,
        skos:Concept,
        dcat:Resource ;
    rdfs:label "Item I595"@en-AU ;
    rdfs:comment "153 ZIM  Interpretation - GraphNodeID: I595"@en-AU ;
    skos:definition "153 ZIM  Interpretation"@en-AU ;
    skos:narrower C1901A00006:593 ;
    skos:prefLabel "Item I595"@en-AU ;
    dcat:accessURL "https://www.legislation.gov.au/C1901A00006/2024-07-01/2024-07-01/text/original/epub/OEBPS/document_2/document_2.html#_Toc172624350"^^xsd:anyURI .

C1901A00006:597 a legcons:Item,
        skos:Concept,
        dcat:Resource ;
    rdfs:label "Item I597"@en-AU ;
    rdfs:comment "153 ZIN  Goods wholly obtained or produced entirely in Peru or in Peru and Australia - GraphNodeID: I597"@en-AU ;
    skos:definition "153 ZIN  Goods wholly obtained or produced entirely in Peru or in Peru and Australia"@en-AU ;
    skos:narrower C1901A00006:596 ;
    skos:prefLabel "Item I597"@en-AU ;
    dcat:accessURL "https://www.legislation.gov.au/C1901A00006/2024-07-01/2024-07-01/text/original/epub/OEBPS/document_2/document_2.html#_Toc172624352"^^xsd:anyURI .

C1901A00006:599 a legcons:Item,
        skos:Concept,
        dcat:Resource ;
    rdfs:label "Item I599"@en-AU ;
    rdfs:comment "153 ZIO  Goods produced in Peru or in Peru and Australia from originating materials - GraphNodeID: I599"@en-AU ;
    skos:definition "153 ZIO  Goods produced in Peru or in Peru and Australia from originating materials"@en-AU ;
    skos:narrower C1901A00006:598 ;
    skos:prefLabel "Item I599"@en-AU ;
    dcat:accessURL "https://www.legislation.gov.au/C1901A00006/2024-07-01/2024-07-01/text/original/epub/OEBPS/document_2/document_2.html#_Toc172624354"^^xsd:anyURI .

C1901A00006:6 a legcons:Item,
        skos:Concept,
        dcat:Resource ;
    rdfs:label "Item I6"@en-AU ;
    rdfs:comment "4 AAA  Members of family - GraphNodeID: I6"@en-AU ;
    skos:definition "4 AAA  Members of family"@en-AU ;
    skos:narrower C1901A00006:2 ;
    skos:prefLabel "Item I6"@en-AU ;
    dcat:accessURL "https://www.legislation.gov.au/C1901A00006/2024-07-01/2024-07-01/text/original/epub/OEBPS/document_1/document_1.html#_Toc172622980"^^xsd:anyURI .

C1901A00006:601 a legcons:Item,
        skos:Concept,
        dcat:Resource ;
    rdfs:label "Item I601"@en-AU ;
    rdfs:comment "153 ZIP  Goods produced in Peru or in Peru and Australia from non originating materials - GraphNodeID: I601"@en-AU ;
    skos:definition "153 ZIP  Goods produced in Peru or in Peru and Australia from non originating materials"@en-AU ;
    skos:narrower C1901A00006:600 ;
    skos:prefLabel "Item I601"@en-AU ;
    dcat:accessURL "https://www.legislation.gov.au/C1901A00006/2024-07-01/2024-07-01/text/original/epub/OEBPS/document_2/document_2.html#_Toc172624356"^^xsd:anyURI .

C1901A00006:602 a legcons:Item,
        skos:Concept,
        dcat:Resource ;
    rdfs:label "Item I602"@en-AU ;
    rdfs:comment "153 ZIQ  Packaging materials and containers - GraphNodeID: I602"@en-AU ;
    skos:definition "153 ZIQ  Packaging materials and containers"@en-AU ;
    skos:narrower C1901A00006:600 ;
    skos:prefLabel "Item I602"@en-AU ;
    dcat:accessURL "https://www.legislation.gov.au/C1901A00006/2024-07-01/2024-07-01/text/original/epub/OEBPS/document_2/document_2.html#_Toc172624357"^^xsd:anyURI .

C1901A00006:604 a legcons:Item,
        skos:Concept,
        dcat:Resource ;
    rdfs:label "Item I604"@en-AU ;
    rdfs:comment "153 ZIR  Goods that are accessories spare parts tools or instructional or other information materials - GraphNodeID: I604"@en-AU ;
    skos:definition "153 ZIR  Goods that are accessories spare parts tools or instructional or other information materials"@en-AU ;
    skos:narrower C1901A00006:603 ;
    skos:prefLabel "Item I604"@en-AU ;
    dcat:accessURL "https://www.legislation.gov.au/C1901A00006/2024-07-01/2024-07-01/text/original/epub/OEBPS/document_2/document_2.html#_Toc172624359"^^xsd:anyURI .

C1901A00006:606 a legcons:Item,
        skos:Concept,
        dcat:Resource ;
    rdfs:label "Item I606"@en-AU ;
    rdfs:comment "153 ZIS  Consignment - GraphNodeID: I606"@en-AU ;
    skos:definition "153 ZIS  Consignment"@en-AU ;
    skos:narrower C1901A00006:605 ;
    skos:prefLabel "Item I606"@en-AU ;
    dcat:accessURL "https://www.legislation.gov.au/C1901A00006/2024-07-01/2024-07-01/text/original/epub/OEBPS/document_2/document_2.html#_Toc172624361"^^xsd:anyURI .

C1901A00006:608 a legcons:Item,
        skos:Concept,
        dcat:Resource ;
    rdfs:label "Item I608"@en-AU ;
    rdfs:comment "153 ZIT  Regulations - GraphNodeID: I608"@en-AU ;
    skos:definition "153 ZIT  Regulations"@en-AU ;
    skos:narrower C1901A00006:607 ;
    skos:prefLabel "Item I608"@en-AU ;
    dcat:accessURL "https://www.legislation.gov.au/C1901A00006/2024-07-01/2024-07-01/text/original/epub/OEBPS/document_2/document_2.html#_Toc172624363"^^xsd:anyURI .

C1901A00006:61 a legcons:Item,
        skos:Concept,
        dcat:Resource ;
    rdfs:label "Item I61"@en-AU ;
    rdfs:comment "50  Prohibition of the importation of goods - GraphNodeID: I61"@en-AU ;
    skos:definition "50  Prohibition of the importation of goods"@en-AU ;
    skos:narrower C1901A00006:60 ;
    skos:prefLabel "Item I61"@en-AU ;
    dcat:accessURL "https://www.legislation.gov.au/C1901A00006/2024-07-01/2024-07-01/text/original/epub/OEBPS/document_1/document_1.html#_Toc172623035"^^xsd:anyURI .

C1901A00006:611 a legcons:Item,
        skos:Concept,
        dcat:Resource ;
    rdfs:label "Item I611"@en-AU ;
    rdfs:comment "153 ZJA  Simplified outline - GraphNodeID: I611"@en-AU ;
    skos:definition "153 ZJA  Simplified outline"@en-AU ;
    skos:narrower C1901A00006:610 ;
    skos:prefLabel "Item I611"@en-AU ;
    dcat:accessURL "https://www.legislation.gov.au/C1901A00006/2024-07-01/2024-07-01/text/original/epub/OEBPS/document_2/document_2.html#_Toc172624366"^^xsd:anyURI .

C1901A00006:612 a legcons:Item,
        skos:Concept,
        dcat:Resource ;
    rdfs:label "Item I612"@en-AU ;
    rdfs:comment "153 ZJB  Interpretation - GraphNodeID: I612"@en-AU ;
    skos:definition "153 ZJB  Interpretation"@en-AU ;
    skos:narrower C1901A00006:610 ;
    skos:prefLabel "Item I612"@en-AU ;
    dcat:accessURL "https://www.legislation.gov.au/C1901A00006/2024-07-01/2024-07-01/text/original/epub/OEBPS/document_2/document_2.html#_Toc172624367"^^xsd:anyURI .

C1901A00006:614 a legcons:Item,
        skos:Concept,
        dcat:Resource ;
    rdfs:label "Item I614"@en-AU ;
    rdfs:comment "153 ZJC  Wholly obtained goods of Chile - GraphNodeID: I614"@en-AU ;
    skos:definition "153 ZJC  Wholly obtained goods of Chile"@en-AU ;
    skos:narrower C1901A00006:613 ;
    skos:prefLabel "Item I614"@en-AU ;
    dcat:accessURL "https://www.legislation.gov.au/C1901A00006/2024-07-01/2024-07-01/text/original/epub/OEBPS/document_2/document_2.html#_Toc172624369"^^xsd:anyURI .

C1901A00006:616 a legcons:Item,
        skos:Concept,
        dcat:Resource ;
    rdfs:label "Item I616"@en-AU ;
    rdfs:comment "153 ZJD  Goods produced in Chile from originating materials - GraphNodeID: I616"@en-AU ;
    skos:definition "153 ZJD  Goods produced in Chile from originating materials"@en-AU ;
    skos:narrower C1901A00006:615 ;
    skos:prefLabel "Item I616"@en-AU ;
    dcat:accessURL "https://www.legislation.gov.au/C1901A00006/2024-07-01/2024-07-01/text/original/epub/OEBPS/document_2/document_2.html#_Toc172624371"^^xsd:anyURI .

C1901A00006:618 a legcons:Item,
        skos:Concept,
        dcat:Resource ;
    rdfs:label "Item I618"@en-AU ;
    rdfs:comment "153 ZJE  Goods produced in Chile or Chile and Australia from non originating materials - GraphNodeID: I618"@en-AU ;
    skos:definition "153 ZJE  Goods produced in Chile or Chile and Australia from non originating materials"@en-AU ;
    skos:narrower C1901A00006:617 ;
    skos:prefLabel "Item I618"@en-AU ;
    dcat:accessURL "https://www.legislation.gov.au/C1901A00006/2024-07-01/2024-07-01/text/original/epub/OEBPS/document_2/document_2.html#_Toc172624373"^^xsd:anyURI .

C1901A00006:619 a legcons:Item,
        skos:Concept,
        dcat:Resource ;
    rdfs:label "Item I619"@en-AU ;
    rdfs:comment "153 ZJF  Packaging materials and containers - GraphNodeID: I619"@en-AU ;
    skos:definition "153 ZJF  Packaging materials and containers"@en-AU ;
    skos:narrower C1901A00006:617 ;
    skos:prefLabel "Item I619"@en-AU ;
    dcat:accessURL "https://www.legislation.gov.au/C1901A00006/2024-07-01/2024-07-01/text/original/epub/OEBPS/document_2/document_2.html#_Toc172624374"^^xsd:anyURI .

C1901A00006:62 a legcons:Item,
        skos:Concept,
        dcat:Resource ;
    rdfs:label "Item I62"@en-AU ;
    rdfs:comment "51  Prohibited imports - GraphNodeID: I62"@en-AU ;
    skos:definition "51  Prohibited imports"@en-AU ;
    skos:narrower C1901A00006:60 ;
    skos:prefLabel "Item I62"@en-AU ;
    dcat:accessURL "https://www.legislation.gov.au/C1901A00006/2024-07-01/2024-07-01/text/original/epub/OEBPS/document_1/document_1.html#_Toc172623036"^^xsd:anyURI .

C1901A00006:621 a legcons:Item,
        skos:Concept,
        dcat:Resource ;
    rdfs:label "Item I621"@en-AU ;
    rdfs:comment "153 ZJG  Goods that are accessories spare parts tools or instructional or other information resources - GraphNodeID: I621"@en-AU ;
    skos:definition "153 ZJG  Goods that are accessories spare parts tools or instructional or other information resources"@en-AU ;
    skos:narrower C1901A00006:620 ;
    skos:prefLabel "Item I621"@en-AU ;
    dcat:accessURL "https://www.legislation.gov.au/C1901A00006/2024-07-01/2024-07-01/text/original/epub/OEBPS/document_2/document_2.html#_Toc172624376"^^xsd:anyURI .

C1901A00006:623 a legcons:Item,
        skos:Concept,
        dcat:Resource ;
    rdfs:label "Item I623"@en-AU ;
    rdfs:comment "153 ZJH  Non qualifying operations - GraphNodeID: I623"@en-AU ;
    skos:definition "153 ZJH  Non qualifying operations"@en-AU ;
    skos:narrower C1901A00006:622 ;
    skos:prefLabel "Item I623"@en-AU ;
    dcat:accessURL "https://www.legislation.gov.au/C1901A00006/2024-07-01/2024-07-01/text/original/epub/OEBPS/document_2/document_2.html#_Toc172624378"^^xsd:anyURI .

C1901A00006:625 a legcons:Item,
        skos:Concept,
        dcat:Resource ;
    rdfs:label "Item I625"@en-AU ;
    rdfs:comment "153 ZJI  Consignment - GraphNodeID: I625"@en-AU ;
    skos:definition "153 ZJI  Consignment"@en-AU ;
    skos:narrower C1901A00006:624 ;
    skos:prefLabel "Item I625"@en-AU ;
    dcat:accessURL "https://www.legislation.gov.au/C1901A00006/2024-07-01/2024-07-01/text/original/epub/OEBPS/document_2/document_2.html#_Toc172624380"^^xsd:anyURI .

C1901A00006:627 a legcons:Item,
        skos:Concept,
        dcat:Resource ;
    rdfs:label "Item I627"@en-AU ;
    rdfs:comment "153 ZJJ  Regulations - GraphNodeID: I627"@en-AU ;
    skos:definition "153 ZJJ  Regulations"@en-AU ;
    skos:narrower C1901A00006:626 ;
    skos:prefLabel "Item I627"@en-AU ;
    dcat:accessURL "https://www.legislation.gov.au/C1901A00006/2024-07-01/2024-07-01/text/original/epub/OEBPS/document_2/document_2.html#_Toc172624382"^^xsd:anyURI .

C1901A00006:63 a legcons:Item,
        skos:Concept,
        dcat:Resource ;
    rdfs:label "Item I63"@en-AU ;
    rdfs:comment "51 A  Certain controlled substances taken to be prohibited imports - GraphNodeID: I63"@en-AU ;
    skos:definition "51 A  Certain controlled substances taken to be prohibited imports"@en-AU ;
    skos:narrower C1901A00006:60 ;
    skos:prefLabel "Item I63"@en-AU ;
    dcat:accessURL "https://www.legislation.gov.au/C1901A00006/2024-07-01/2024-07-01/text/original/epub/OEBPS/document_1/document_1.html#_Toc172623037"^^xsd:anyURI .

C1901A00006:630 a legcons:Item,
        skos:Concept,
        dcat:Resource ;
    rdfs:label "Item I630"@en-AU ;
    rdfs:comment "153 ZKA  Simplified outline - GraphNodeID: I630"@en-AU ;
    skos:definition "153 ZKA  Simplified outline"@en-AU ;
    skos:narrower C1901A00006:629 ;
    skos:prefLabel "Item I630"@en-AU ;
    dcat:accessURL "https://www.legislation.gov.au/C1901A00006/2024-07-01/2024-07-01/text/original/epub/OEBPS/document_2/document_2.html#_Toc172624385"^^xsd:anyURI .

C1901A00006:631 a legcons:Item,
        skos:Concept,
        dcat:Resource ;
    rdfs:label "Item I631"@en-AU ;
    rdfs:comment "153 ZKB  Interpretation - GraphNodeID: I631"@en-AU ;
    skos:definition "153 ZKB  Interpretation"@en-AU ;
    skos:narrower C1901A00006:629 ;
    skos:prefLabel "Item I631"@en-AU ;
    dcat:accessURL "https://www.legislation.gov.au/C1901A00006/2024-07-01/2024-07-01/text/original/epub/OEBPS/document_2/document_2.html#_Toc172624386"^^xsd:anyURI .

C1901A00006:633 a legcons:Item,
        skos:Concept,
        dcat:Resource ;
    rdfs:label "Item I633"@en-AU ;
    rdfs:comment "153 ZKC  Wholly obtained goods of a Party - GraphNodeID: I633"@en-AU ;
    skos:definition "153 ZKC  Wholly obtained goods of a Party"@en-AU ;
    skos:narrower C1901A00006:632 ;
    skos:prefLabel "Item I633"@en-AU ;
    dcat:accessURL "https://www.legislation.gov.au/C1901A00006/2024-07-01/2024-07-01/text/original/epub/OEBPS/document_2/document_2.html#_Toc172624388"^^xsd:anyURI .

C1901A00006:635 a legcons:Item,
        skos:Concept,
        dcat:Resource ;
    rdfs:label "Item I635"@en-AU ;
    rdfs:comment "153 ZKD  Goods produced from originating materials - GraphNodeID: I635"@en-AU ;
    skos:definition "153 ZKD  Goods produced from originating materials"@en-AU ;
    skos:narrower C1901A00006:634 ;
    skos:prefLabel "Item I635"@en-AU ;
    dcat:accessURL "https://www.legislation.gov.au/C1901A00006/2024-07-01/2024-07-01/text/original/epub/OEBPS/document_2/document_2.html#_Toc172624390"^^xsd:anyURI .

C1901A00006:637 a legcons:Item,
        skos:Concept,
        dcat:Resource ;
    rdfs:label "Item I637"@en-AU ;
    rdfs:comment "153 ZKE  Goods produced from non originating materials - GraphNodeID: I637"@en-AU ;
    skos:definition "153 ZKE  Goods produced from non originating materials"@en-AU ;
    skos:narrower C1901A00006:636 ;
    skos:prefLabel "Item I637"@en-AU ;
    dcat:accessURL "https://www.legislation.gov.au/C1901A00006/2024-07-01/2024-07-01/text/original/epub/OEBPS/document_2/document_2.html#_Toc172624392"^^xsd:anyURI .

C1901A00006:638 a legcons:Item,
        skos:Concept,
        dcat:Resource ;
    rdfs:label "Item I638"@en-AU ;
    rdfs:comment "153 ZKG  Non qualifying operations or processes - GraphNodeID: I638"@en-AU ;
    skos:definition "153 ZKG  Non qualifying operations or processes"@en-AU ;
    skos:narrower C1901A00006:636 ;
    skos:prefLabel "Item I638"@en-AU ;
    dcat:accessURL "https://www.legislation.gov.au/C1901A00006/2024-07-01/2024-07-01/text/original/epub/OEBPS/document_2/document_2.html#_Toc172624393"^^xsd:anyURI .

C1901A00006:639 a legcons:Item,
        skos:Concept,
        dcat:Resource ;
    rdfs:label "Item I639"@en-AU ;
    rdfs:comment "153 ZKH  Packaging materials and containers - GraphNodeID: I639"@en-AU ;
    skos:definition "153 ZKH  Packaging materials and containers"@en-AU ;
    skos:narrower C1901A00006:636 ;
    skos:prefLabel "Item I639"@en-AU ;
    dcat:accessURL "https://www.legislation.gov.au/C1901A00006/2024-07-01/2024-07-01/text/original/epub/OEBPS/document_2/document_2.html#_Toc172624394"^^xsd:anyURI .

C1901A00006:64 a legcons:Item,
        skos:Concept,
        dcat:Resource ;
    rdfs:label "Item I64"@en-AU ;
    rdfs:comment "52  Invalidation of licence permission etc for false or misleading information - GraphNodeID: I64"@en-AU ;
    skos:definition "52  Invalidation of licence permission etc for false or misleading information"@en-AU ;
    skos:narrower C1901A00006:60 ;
    skos:prefLabel "Item I64"@en-AU ;
    dcat:accessURL "https://www.legislation.gov.au/C1901A00006/2024-07-01/2024-07-01/text/original/epub/OEBPS/document_1/document_1.html#_Toc172623038"^^xsd:anyURI .

C1901A00006:641 a legcons:Item,
        skos:Concept,
        dcat:Resource ;
    rdfs:label "Item I641"@en-AU ;
    rdfs:comment "153 ZKI  Goods that are accessories spare parts tools or instructional or other information materials - GraphNodeID: I641"@en-AU ;
    skos:definition "153 ZKI  Goods that are accessories spare parts tools or instructional or other information materials"@en-AU ;
    skos:narrower C1901A00006:640 ;
    skos:prefLabel "Item I641"@en-AU ;
    dcat:accessURL "https://www.legislation.gov.au/C1901A00006/2024-07-01/2024-07-01/text/original/epub/OEBPS/document_2/document_2.html#_Toc172624396"^^xsd:anyURI .

C1901A00006:643 a legcons:Item,
        skos:Concept,
        dcat:Resource ;
    rdfs:label "Item I643"@en-AU ;
    rdfs:comment "153 ZKJ  Consignment - GraphNodeID: I643"@en-AU ;
    skos:definition "153 ZKJ  Consignment"@en-AU ;
    skos:narrower C1901A00006:642 ;
    skos:prefLabel "Item I643"@en-AU ;
    dcat:accessURL "https://www.legislation.gov.au/C1901A00006/2024-07-01/2024-07-01/text/original/epub/OEBPS/document_2/document_2.html#_Toc172624398"^^xsd:anyURI .

C1901A00006:645 a legcons:Item,
        skos:Concept,
        dcat:Resource ;
    rdfs:label "Item I645"@en-AU ;
    rdfs:comment "153 ZKJA  Regulations - GraphNodeID: I645"@en-AU ;
    skos:definition "153 ZKJA  Regulations"@en-AU ;
    skos:narrower C1901A00006:644 ;
    skos:prefLabel "Item I645"@en-AU ;
    dcat:accessURL "https://www.legislation.gov.au/C1901A00006/2024-07-01/2024-07-01/text/original/epub/OEBPS/document_2/document_2.html#_Toc172624400"^^xsd:anyURI .

C1901A00006:648 a legcons:Item,
        skos:Concept,
        dcat:Resource ;
    rdfs:label "Item I648"@en-AU ;
    rdfs:comment "153 ZKK  Simplified outline of this Division - GraphNodeID: I648"@en-AU ;
    skos:definition "153 ZKK  Simplified outline of this Division"@en-AU ;
    skos:narrower C1901A00006:647 ;
    skos:prefLabel "Item I648"@en-AU ;
    dcat:accessURL "https://www.legislation.gov.au/C1901A00006/2024-07-01/2024-07-01/text/original/epub/OEBPS/document_2/document_2.html#_Toc172624403"^^xsd:anyURI .

C1901A00006:649 a legcons:Item,
        skos:Concept,
        dcat:Resource ;
    rdfs:label "Item I649"@en-AU ;
    rdfs:comment "153 ZKL  Interpretation - GraphNodeID: I649"@en-AU ;
    skos:definition "153 ZKL  Interpretation"@en-AU ;
    skos:narrower C1901A00006:647 ;
    skos:prefLabel "Item I649"@en-AU ;
    dcat:accessURL "https://www.legislation.gov.au/C1901A00006/2024-07-01/2024-07-01/text/original/epub/OEBPS/document_2/document_2.html#_Toc172624404"^^xsd:anyURI .

C1901A00006:651 a legcons:Item,
        skos:Concept,
        dcat:Resource ;
    rdfs:label "Item I651"@en-AU ;
    rdfs:comment "153 ZKM  Goods wholly obtained or produced in a Party - GraphNodeID: I651"@en-AU ;
    skos:definition "153 ZKM  Goods wholly obtained or produced in a Party"@en-AU ;
    skos:narrower C1901A00006:650 ;
    skos:prefLabel "Item I651"@en-AU ;
    dcat:accessURL "https://www.legislation.gov.au/C1901A00006/2024-07-01/2024-07-01/text/original/epub/OEBPS/document_2/document_2.html#_Toc172624406"^^xsd:anyURI .

C1901A00006:653 a legcons:Item,
        skos:Concept,
        dcat:Resource ;
    rdfs:label "Item I653"@en-AU ;
    rdfs:comment "153 ZKN  Goods produced from originating materials - GraphNodeID: I653"@en-AU ;
    skos:definition "153 ZKN  Goods produced from originating materials"@en-AU ;
    skos:narrower C1901A00006:652 ;
    skos:prefLabel "Item I653"@en-AU ;
    dcat:accessURL "https://www.legislation.gov.au/C1901A00006/2024-07-01/2024-07-01/text/original/epub/OEBPS/document_2/document_2.html#_Toc172624408"^^xsd:anyURI .

C1901A00006:655 a legcons:Item,
        skos:Concept,
        dcat:Resource ;
    rdfs:label "Item I655"@en-AU ;
    rdfs:comment "153 ZKO  Goods produced from non originating materials - GraphNodeID: I655"@en-AU ;
    skos:definition "153 ZKO  Goods produced from non originating materials"@en-AU ;
    skos:narrower C1901A00006:654 ;
    skos:prefLabel "Item I655"@en-AU ;
    dcat:accessURL "https://www.legislation.gov.au/C1901A00006/2024-07-01/2024-07-01/text/original/epub/OEBPS/document_2/document_2.html#_Toc172624410"^^xsd:anyURI .

C1901A00006:656 a legcons:Item,
        skos:Concept,
        dcat:Resource ;
    rdfs:label "Item I656"@en-AU ;
    rdfs:comment "153 ZKP  Packaging materials and containers - GraphNodeID: I656"@en-AU ;
    skos:definition "153 ZKP  Packaging materials and containers"@en-AU ;
    skos:narrower C1901A00006:654 ;
    skos:prefLabel "Item I656"@en-AU ;
    dcat:accessURL "https://www.legislation.gov.au/C1901A00006/2024-07-01/2024-07-01/text/original/epub/OEBPS/document_2/document_2.html#_Toc172624411"^^xsd:anyURI .

C1901A00006:658 a legcons:Item,
        skos:Concept,
        dcat:Resource ;
    rdfs:label "Item I658"@en-AU ;
    rdfs:comment "153 ZKQ  Goods that are accessories spare parts tools or instructional or other information materials - GraphNodeID: I658"@en-AU ;
    skos:definition "153 ZKQ  Goods that are accessories spare parts tools or instructional or other information materials"@en-AU ;
    skos:narrower C1901A00006:657 ;
    skos:prefLabel "Item I658"@en-AU ;
    dcat:accessURL "https://www.legislation.gov.au/C1901A00006/2024-07-01/2024-07-01/text/original/epub/OEBPS/document_2/document_2.html#_Toc172624413"^^xsd:anyURI .

C1901A00006:66 a legcons:Item,
        skos:Concept,
        dcat:Resource ;
    rdfs:label "Item I66"@en-AU ;
    rdfs:comment "58  Ships and aircraft to enter ports or airports - GraphNodeID: I66"@en-AU ;
    skos:definition "58  Ships and aircraft to enter ports or airports"@en-AU ;
    skos:narrower C1901A00006:65 ;
    skos:prefLabel "Item I66"@en-AU ;
    dcat:accessURL "https://www.legislation.gov.au/C1901A00006/2024-07-01/2024-07-01/text/original/epub/OEBPS/document_1/document_1.html#_Toc172623040"^^xsd:anyURI .

C1901A00006:660 a legcons:Item,
        skos:Concept,
        dcat:Resource ;
    rdfs:label "Item I660"@en-AU ;
    rdfs:comment "153 ZKR  Consignment - GraphNodeID: I660"@en-AU ;
    skos:definition "153 ZKR  Consignment"@en-AU ;
    skos:narrower C1901A00006:659 ;
    skos:prefLabel "Item I660"@en-AU ;
    dcat:accessURL "https://www.legislation.gov.au/C1901A00006/2024-07-01/2024-07-01/text/original/epub/OEBPS/document_2/document_2.html#_Toc172624415"^^xsd:anyURI .

C1901A00006:662 a legcons:Item,
        skos:Concept,
        dcat:Resource ;
    rdfs:label "Item I662"@en-AU ;
    rdfs:comment "153 ZKS  Regulations - GraphNodeID: I662"@en-AU ;
    skos:definition "153 ZKS  Regulations"@en-AU ;
    skos:narrower C1901A00006:661 ;
    skos:prefLabel "Item I662"@en-AU ;
    dcat:accessURL "https://www.legislation.gov.au/C1901A00006/2024-07-01/2024-07-01/text/original/epub/OEBPS/document_2/document_2.html#_Toc172624417"^^xsd:anyURI .

C1901A00006:665 a legcons:Item,
        skos:Concept,
        dcat:Resource ;
    rdfs:label "Item I665"@en-AU ;
    rdfs:comment "153 ZKT  Simplified outline of this Division - GraphNodeID: I665"@en-AU ;
    skos:definition "153 ZKT  Simplified outline of this Division"@en-AU ;
    skos:narrower C1901A00006:664 ;
    skos:prefLabel "Item I665"@en-AU ;
    dcat:accessURL "https://www.legislation.gov.au/C1901A00006/2024-07-01/2024-07-01/text/original/epub/OEBPS/document_2/document_2.html#_Toc172624420"^^xsd:anyURI .

C1901A00006:666 a legcons:Item,
        skos:Concept,
        dcat:Resource ;
    rdfs:label "Item I666"@en-AU ;
    rdfs:comment "153 ZKU  Interpretation - GraphNodeID: I666"@en-AU ;
    skos:definition "153 ZKU  Interpretation"@en-AU ;
    skos:narrower C1901A00006:664 ;
    skos:prefLabel "Item I666"@en-AU ;
    dcat:accessURL "https://www.legislation.gov.au/C1901A00006/2024-07-01/2024-07-01/text/original/epub/OEBPS/document_2/document_2.html#_Toc172624421"^^xsd:anyURI .

C1901A00006:668 a legcons:Item,
        skos:Concept,
        dcat:Resource ;
    rdfs:label "Item I668"@en-AU ;
    rdfs:comment "153 ZKV  Goods wholly obtained or produced entirely in the territory of one or more of the Parties - GraphNodeID: I668"@en-AU ;
    skos:definition "153 ZKV  Goods wholly obtained or produced entirely in the territory of one or more of the Parties"@en-AU ;
    skos:narrower C1901A00006:667 ;
    skos:prefLabel "Item I668"@en-AU ;
    dcat:accessURL "https://www.legislation.gov.au/C1901A00006/2024-07-01/2024-07-01/text/original/epub/OEBPS/document_2/document_2.html#_Toc172624423"^^xsd:anyURI .

C1901A00006:67 a legcons:Item,
        skos:Concept,
        dcat:Resource ;
    rdfs:label "Item I67"@en-AU ;
    rdfs:comment "58 A  Direct journeys between installations and external places prohibited - GraphNodeID: I67"@en-AU ;
    skos:definition "58 A  Direct journeys between installations and external places prohibited"@en-AU ;
    skos:narrower C1901A00006:65 ;
    skos:prefLabel "Item I67"@en-AU ;
    dcat:accessURL "https://www.legislation.gov.au/C1901A00006/2024-07-01/2024-07-01/text/original/epub/OEBPS/document_1/document_1.html#_Toc172623041"^^xsd:anyURI .

C1901A00006:670 a legcons:Item,
        skos:Concept,
        dcat:Resource ;
    rdfs:label "Item I670"@en-AU ;
    rdfs:comment "153 ZKW  Goods produced from originating materials - GraphNodeID: I670"@en-AU ;
    skos:definition "153 ZKW  Goods produced from originating materials"@en-AU ;
    skos:narrower C1901A00006:669 ;
    skos:prefLabel "Item I670"@en-AU ;
    dcat:accessURL "https://www.legislation.gov.au/C1901A00006/2024-07-01/2024-07-01/text/original/epub/OEBPS/document_2/document_2.html#_Toc172624425"^^xsd:anyURI .

C1901A00006:672 a legcons:Item,
        skos:Concept,
        dcat:Resource ;
    rdfs:label "Item I672"@en-AU ;
    rdfs:comment "153 ZKX  Goods produced from non originating materials - GraphNodeID: I672"@en-AU ;
    skos:definition "153 ZKX  Goods produced from non originating materials"@en-AU ;
    skos:narrower C1901A00006:671 ;
    skos:prefLabel "Item I672"@en-AU ;
    dcat:accessURL "https://www.legislation.gov.au/C1901A00006/2024-07-01/2024-07-01/text/original/epub/OEBPS/document_2/document_2.html#_Toc172624427"^^xsd:anyURI .

C1901A00006:673 a legcons:Item,
        skos:Concept,
        dcat:Resource ;
    rdfs:label "Item I673"@en-AU ;
    rdfs:comment "153 ZKY  Packaging materials and containers - GraphNodeID: I673"@en-AU ;
    skos:definition "153 ZKY  Packaging materials and containers"@en-AU ;
    skos:narrower C1901A00006:671 ;
    skos:prefLabel "Item I673"@en-AU ;
    dcat:accessURL "https://www.legislation.gov.au/C1901A00006/2024-07-01/2024-07-01/text/original/epub/OEBPS/document_2/document_2.html#_Toc172624428"^^xsd:anyURI .

C1901A00006:675 a legcons:Item,
        skos:Concept,
        dcat:Resource ;
    rdfs:label "Item I675"@en-AU ;
    rdfs:comment "153 ZKZ  Goods that are accessories spare parts tools or instructional or other information materials - GraphNodeID: I675"@en-AU ;
    skos:definition "153 ZKZ  Goods that are accessories spare parts tools or instructional or other information materials"@en-AU ;
    skos:narrower C1901A00006:674 ;
    skos:prefLabel "Item I675"@en-AU ;
    dcat:accessURL "https://www.legislation.gov.au/C1901A00006/2024-07-01/2024-07-01/text/original/epub/OEBPS/document_2/document_2.html#_Toc172624430"^^xsd:anyURI .

C1901A00006:677 a legcons:Item,
        skos:Concept,
        dcat:Resource ;
    rdfs:label "Item I677"@en-AU ;
    rdfs:comment "153 ZKZA  Consignment - GraphNodeID: I677"@en-AU ;
    skos:definition "153 ZKZA  Consignment"@en-AU ;
    skos:narrower C1901A00006:676 ;
    skos:prefLabel "Item I677"@en-AU ;
    dcat:accessURL "https://www.legislation.gov.au/C1901A00006/2024-07-01/2024-07-01/text/original/epub/OEBPS/document_2/document_2.html#_Toc172624432"^^xsd:anyURI .

C1901A00006:679 a legcons:Item,
        skos:Concept,
        dcat:Resource ;
    rdfs:label "Item I679"@en-AU ;
    rdfs:comment "153 ZKZB  Regulations - GraphNodeID: I679"@en-AU ;
    skos:definition "153 ZKZB  Regulations"@en-AU ;
    skos:narrower C1901A00006:678 ;
    skos:prefLabel "Item I679"@en-AU ;
    dcat:accessURL "https://www.legislation.gov.au/C1901A00006/2024-07-01/2024-07-01/text/original/epub/OEBPS/document_2/document_2.html#_Toc172624434"^^xsd:anyURI .

C1901A00006:68 a legcons:Item,
        skos:Concept,
        dcat:Resource ;
    rdfs:label "Item I68"@en-AU ;
    rdfs:comment "58 B  Direct journeys between certain resources installations and external places prohibited - GraphNodeID: I68"@en-AU ;
    skos:definition "58 B  Direct journeys between certain resources installations and external places prohibited"@en-AU ;
    skos:narrower C1901A00006:65 ;
    skos:prefLabel "Item I68"@en-AU ;
    dcat:accessURL "https://www.legislation.gov.au/C1901A00006/2024-07-01/2024-07-01/text/original/epub/OEBPS/document_1/document_1.html#_Toc172623042"^^xsd:anyURI .

C1901A00006:682 a legcons:Item,
        skos:Concept,
        dcat:Resource ;
    rdfs:label "Item I682"@en-AU ;
    rdfs:comment "153 ZLA  Simplified outline - GraphNodeID: I682"@en-AU ;
    skos:definition "153 ZLA  Simplified outline"@en-AU ;
    skos:narrower C1901A00006:681 ;
    skos:prefLabel "Item I682"@en-AU ;
    dcat:accessURL "https://www.legislation.gov.au/C1901A00006/2024-07-01/2024-07-01/text/original/epub/OEBPS/document_2/document_2.html#_Toc172624437"^^xsd:anyURI .

C1901A00006:683 a legcons:Item,
        skos:Concept,
        dcat:Resource ;
    rdfs:label "Item I683"@en-AU ;
    rdfs:comment "153 ZLB  Interpretation - GraphNodeID: I683"@en-AU ;
    skos:definition "153 ZLB  Interpretation"@en-AU ;
    skos:narrower C1901A00006:681 ;
    skos:prefLabel "Item I683"@en-AU ;
    dcat:accessURL "https://www.legislation.gov.au/C1901A00006/2024-07-01/2024-07-01/text/original/epub/OEBPS/document_2/document_2.html#_Toc172624438"^^xsd:anyURI .

C1901A00006:685 a legcons:Item,
        skos:Concept,
        dcat:Resource ;
    rdfs:label "Item I685"@en-AU ;
    rdfs:comment "153 ZLC  Goods wholly obtained or produced in Malaysia or in Malaysia and Australia - GraphNodeID: I685"@en-AU ;
    skos:definition "153 ZLC  Goods wholly obtained or produced in Malaysia or in Malaysia and Australia"@en-AU ;
    skos:narrower C1901A00006:684 ;
    skos:prefLabel "Item I685"@en-AU ;
    dcat:accessURL "https://www.legislation.gov.au/C1901A00006/2024-07-01/2024-07-01/text/original/epub/OEBPS/document_2/document_2.html#_Toc172624440"^^xsd:anyURI .

C1901A00006:687 a legcons:Item,
        skos:Concept,
        dcat:Resource ;
    rdfs:label "Item I687"@en-AU ;
    rdfs:comment "153 ZLD  Goods produced in Malaysia or in Malaysia and Australia from originating materials - GraphNodeID: I687"@en-AU ;
    skos:definition "153 ZLD  Goods produced in Malaysia or in Malaysia and Australia from originating materials"@en-AU ;
    skos:narrower C1901A00006:686 ;
    skos:prefLabel "Item I687"@en-AU ;
    dcat:accessURL "https://www.legislation.gov.au/C1901A00006/2024-07-01/2024-07-01/text/original/epub/OEBPS/document_2/document_2.html#_Toc172624442"^^xsd:anyURI .

C1901A00006:689 a legcons:Item,
        skos:Concept,
        dcat:Resource ;
    rdfs:label "Item I689"@en-AU ;
    rdfs:comment "153 ZLE  Goods produced in Malaysia or in Malaysia and Australia from non originating materials - GraphNodeID: I689"@en-AU ;
    skos:definition "153 ZLE  Goods produced in Malaysia or in Malaysia and Australia from non originating materials"@en-AU ;
    skos:narrower C1901A00006:688 ;
    skos:prefLabel "Item I689"@en-AU ;
    dcat:accessURL "https://www.legislation.gov.au/C1901A00006/2024-07-01/2024-07-01/text/original/epub/OEBPS/document_2/document_2.html#_Toc172624444"^^xsd:anyURI .

C1901A00006:69 a legcons:Item,
        skos:Concept,
        dcat:Resource ;
    rdfs:label "Item I69"@en-AU ;
    rdfs:comment "60  Boarding stations - GraphNodeID: I69"@en-AU ;
    skos:definition "60  Boarding stations"@en-AU ;
    skos:narrower C1901A00006:65 ;
    skos:prefLabel "Item I69"@en-AU ;
    dcat:accessURL "https://www.legislation.gov.au/C1901A00006/2024-07-01/2024-07-01/text/original/epub/OEBPS/document_1/document_1.html#_Toc172623043"^^xsd:anyURI .

C1901A00006:690 a legcons:Item,
        skos:Concept,
        dcat:Resource ;
    rdfs:label "Item I690"@en-AU ;
    rdfs:comment "153 ZLF  Packaging materials and containers - GraphNodeID: I690"@en-AU ;
    skos:definition "153 ZLF  Packaging materials and containers"@en-AU ;
    skos:narrower C1901A00006:688 ;
    skos:prefLabel "Item I690"@en-AU ;
    dcat:accessURL "https://www.legislation.gov.au/C1901A00006/2024-07-01/2024-07-01/text/original/epub/OEBPS/document_2/document_2.html#_Toc172624445"^^xsd:anyURI .

C1901A00006:691 a legcons:Item,
        skos:Concept,
        dcat:Resource ;
    rdfs:label "Item I691"@en-AU ;
    rdfs:comment "153 ZLG  Non qualifying operations - GraphNodeID: I691"@en-AU ;
    skos:definition "153 ZLG  Non qualifying operations"@en-AU ;
    skos:narrower C1901A00006:688 ;
    skos:prefLabel "Item I691"@en-AU ;
    dcat:accessURL "https://www.legislation.gov.au/C1901A00006/2024-07-01/2024-07-01/text/original/epub/OEBPS/document_2/document_2.html#_Toc172624446"^^xsd:anyURI .

C1901A00006:693 a legcons:Item,
        skos:Concept,
        dcat:Resource ;
    rdfs:label "Item I693"@en-AU ;
    rdfs:comment "153 ZLH  Goods that are accessories spare parts tools or instructional or other information materials - GraphNodeID: I693"@en-AU ;
    skos:definition "153 ZLH  Goods that are accessories spare parts tools or instructional or other information materials"@en-AU ;
    skos:narrower C1901A00006:692 ;
    skos:prefLabel "Item I693"@en-AU ;
    dcat:accessURL "https://www.legislation.gov.au/C1901A00006/2024-07-01/2024-07-01/text/original/epub/OEBPS/document_2/document_2.html#_Toc172624448"^^xsd:anyURI .

C1901A00006:695 a legcons:Item,
        skos:Concept,
        dcat:Resource ;
    rdfs:label "Item I695"@en-AU ;
    rdfs:comment "153 ZLI  Consignment - GraphNodeID: I695"@en-AU ;
    skos:definition "153 ZLI  Consignment"@en-AU ;
    skos:narrower C1901A00006:694 ;
    skos:prefLabel "Item I695"@en-AU ;
    dcat:accessURL "https://www.legislation.gov.au/C1901A00006/2024-07-01/2024-07-01/text/original/epub/OEBPS/document_2/document_2.html#_Toc172624450"^^xsd:anyURI .

C1901A00006:697 a legcons:Item,
        skos:Concept,
        dcat:Resource ;
    rdfs:label "Item I697"@en-AU ;
    rdfs:comment "153 ZLJ  Regulations - GraphNodeID: I697"@en-AU ;
    skos:definition "153 ZLJ  Regulations"@en-AU ;
    skos:narrower C1901A00006:696 ;
    skos:prefLabel "Item I697"@en-AU ;
    dcat:accessURL "https://www.legislation.gov.au/C1901A00006/2024-07-01/2024-07-01/text/original/epub/OEBPS/document_2/document_2.html#_Toc172624452"^^xsd:anyURI .

C1901A00006:7 a legcons:Item,
        skos:Concept,
        dcat:Resource ;
    rdfs:label "Item I7"@en-AU ;
    rdfs:comment "4 AA  Act not to apply so as to exceed Commonwealth power - GraphNodeID: I7"@en-AU ;
    skos:definition "4 AA  Act not to apply so as to exceed Commonwealth power"@en-AU ;
    skos:narrower C1901A00006:2 ;
    skos:prefLabel "Item I7"@en-AU ;
    dcat:accessURL "https://www.legislation.gov.au/C1901A00006/2024-07-01/2024-07-01/text/original/epub/OEBPS/document_1/document_1.html#_Toc172622981"^^xsd:anyURI .

C1901A00006:70 a legcons:Item,
        skos:Concept,
        dcat:Resource ;
    rdfs:label "Item I70"@en-AU ;
    rdfs:comment "61  Facility for boarding - GraphNodeID: I70"@en-AU ;
    skos:definition "61  Facility for boarding"@en-AU ;
    skos:narrower C1901A00006:65 ;
    skos:prefLabel "Item I70"@en-AU ;
    dcat:accessURL "https://www.legislation.gov.au/C1901A00006/2024-07-01/2024-07-01/text/original/epub/OEBPS/document_1/document_1.html#_Toc172623044"^^xsd:anyURI .

C1901A00006:700 a legcons:Item,
        skos:Concept,
        dcat:Resource ;
    rdfs:label "Item I700"@en-AU ;
    rdfs:comment "153 ZLJA  Simplified outline of this Division - GraphNodeID: I700"@en-AU ;
    skos:definition "153 ZLJA  Simplified outline of this Division"@en-AU ;
    skos:narrower C1901A00006:699 ;
    skos:prefLabel "Item I700"@en-AU ;
    dcat:accessURL "https://www.legislation.gov.au/C1901A00006/2024-07-01/2024-07-01/text/original/epub/OEBPS/document_2/document_2.html#_Toc172624455"^^xsd:anyURI .

C1901A00006:701 a legcons:Item,
        skos:Concept,
        dcat:Resource ;
    rdfs:label "Item I701"@en-AU ;
    rdfs:comment "153 ZLK  Interpretation - GraphNodeID: I701"@en-AU ;
    skos:definition "153 ZLK  Interpretation"@en-AU ;
    skos:narrower C1901A00006:699 ;
    skos:prefLabel "Item I701"@en-AU ;
    dcat:accessURL "https://www.legislation.gov.au/C1901A00006/2024-07-01/2024-07-01/text/original/epub/OEBPS/document_2/document_2.html#_Toc172624456"^^xsd:anyURI .

C1901A00006:703 a legcons:Item,
        skos:Concept,
        dcat:Resource ;
    rdfs:label "Item I703"@en-AU ;
    rdfs:comment "153 ZLL  Goods wholly obtained or produced in Indonesia - GraphNodeID: I703"@en-AU ;
    skos:definition "153 ZLL  Goods wholly obtained or produced in Indonesia"@en-AU ;
    skos:narrower C1901A00006:702 ;
    skos:prefLabel "Item I703"@en-AU ;
    dcat:accessURL "https://www.legislation.gov.au/C1901A00006/2024-07-01/2024-07-01/text/original/epub/OEBPS/document_2/document_2.html#_Toc172624458"^^xsd:anyURI .

C1901A00006:705 a legcons:Item,
        skos:Concept,
        dcat:Resource ;
    rdfs:label "Item I705"@en-AU ;
    rdfs:comment "153 ZLM  Goods produced in Indonesia from originating materials - GraphNodeID: I705"@en-AU ;
    skos:definition "153 ZLM  Goods produced in Indonesia from originating materials"@en-AU ;
    skos:narrower C1901A00006:704 ;
    skos:prefLabel "Item I705"@en-AU ;
    dcat:accessURL "https://www.legislation.gov.au/C1901A00006/2024-07-01/2024-07-01/text/original/epub/OEBPS/document_2/document_2.html#_Toc172624460"^^xsd:anyURI .

C1901A00006:707 a legcons:Item,
        skos:Concept,
        dcat:Resource ;
    rdfs:label "Item I707"@en-AU ;
    rdfs:comment "153 ZLN  Goods produced in Indonesia or in Indonesia and Australia from non originating materials - GraphNodeID: I707"@en-AU ;
    skos:definition "153 ZLN  Goods produced in Indonesia or in Indonesia and Australia from non originating materials"@en-AU ;
    skos:narrower C1901A00006:706 ;
    skos:prefLabel "Item I707"@en-AU ;
    dcat:accessURL "https://www.legislation.gov.au/C1901A00006/2024-07-01/2024-07-01/text/original/epub/OEBPS/document_2/document_2.html#_Toc172624462"^^xsd:anyURI .

C1901A00006:708 a legcons:Item,
        skos:Concept,
        dcat:Resource ;
    rdfs:label "Item I708"@en-AU ;
    rdfs:comment "153 ZLO  Packaging materials and containers - GraphNodeID: I708"@en-AU ;
    skos:definition "153 ZLO  Packaging materials and containers"@en-AU ;
    skos:narrower C1901A00006:706 ;
    skos:prefLabel "Item I708"@en-AU ;
    dcat:accessURL "https://www.legislation.gov.au/C1901A00006/2024-07-01/2024-07-01/text/original/epub/OEBPS/document_2/document_2.html#_Toc172624463"^^xsd:anyURI .

C1901A00006:71 a legcons:Item,
        skos:Concept,
        dcat:Resource ;
    rdfs:label "Item I71"@en-AU ;
    rdfs:comment "61 A  Owner or operator of port etc to facilitate boarding - GraphNodeID: I71"@en-AU ;
    skos:definition "61 A  Owner or operator of port etc to facilitate boarding"@en-AU ;
    skos:narrower C1901A00006:65 ;
    skos:prefLabel "Item I71"@en-AU ;
    dcat:accessURL "https://www.legislation.gov.au/C1901A00006/2024-07-01/2024-07-01/text/original/epub/OEBPS/document_1/document_1.html#_Toc172623045"^^xsd:anyURI .

C1901A00006:710 a legcons:Item,
        skos:Concept,
        dcat:Resource ;
    rdfs:label "Item I710"@en-AU ;
    rdfs:comment "153 ZLP  Consignment - GraphNodeID: I710"@en-AU ;
    skos:definition "153 ZLP  Consignment"@en-AU ;
    skos:narrower C1901A00006:709 ;
    skos:prefLabel "Item I710"@en-AU ;
    dcat:accessURL "https://www.legislation.gov.au/C1901A00006/2024-07-01/2024-07-01/text/original/epub/OEBPS/document_2/document_2.html#_Toc172624465"^^xsd:anyURI .

C1901A00006:711 a legcons:Item,
        skos:Concept,
        dcat:Resource ;
    rdfs:label "Item I711"@en-AU ;
    rdfs:comment "153 ZLQ  Exhibition - GraphNodeID: I711"@en-AU ;
    skos:definition "153 ZLQ  Exhibition"@en-AU ;
    skos:narrower C1901A00006:709 ;
    skos:prefLabel "Item I711"@en-AU ;
    dcat:accessURL "https://www.legislation.gov.au/C1901A00006/2024-07-01/2024-07-01/text/original/epub/OEBPS/document_2/document_2.html#_Toc172624466"^^xsd:anyURI .

C1901A00006:713 a legcons:Item,
        skos:Concept,
        dcat:Resource ;
    rdfs:label "Item I713"@en-AU ;
    rdfs:comment "153 ZLR  Regulations - GraphNodeID: I713"@en-AU ;
    skos:definition "153 ZLR  Regulations"@en-AU ;
    skos:narrower C1901A00006:712 ;
    skos:prefLabel "Item I713"@en-AU ;
    dcat:accessURL "https://www.legislation.gov.au/C1901A00006/2024-07-01/2024-07-01/text/original/epub/OEBPS/document_2/document_2.html#_Toc172624468"^^xsd:anyURI .

C1901A00006:716 a legcons:Item,
        skos:Concept,
        dcat:Resource ;
    rdfs:label "Item I716"@en-AU ;
    rdfs:comment "153 ZMA  Simplified outline of this Division - GraphNodeID: I716"@en-AU ;
    skos:definition "153 ZMA  Simplified outline of this Division"@en-AU ;
    skos:narrower C1901A00006:715 ;
    skos:prefLabel "Item I716"@en-AU ;
    dcat:accessURL "https://www.legislation.gov.au/C1901A00006/2024-07-01/2024-07-01/text/original/epub/OEBPS/document_2/document_2.html#_Toc172624471"^^xsd:anyURI .

C1901A00006:717 a legcons:Item,
        skos:Concept,
        dcat:Resource ;
    rdfs:label "Item I717"@en-AU ;
    rdfs:comment "153 ZMB  Interpretation - GraphNodeID: I717"@en-AU ;
    skos:definition "153 ZMB  Interpretation"@en-AU ;
    skos:narrower C1901A00006:715 ;
    skos:prefLabel "Item I717"@en-AU ;
    dcat:accessURL "https://www.legislation.gov.au/C1901A00006/2024-07-01/2024-07-01/text/original/epub/OEBPS/document_2/document_2.html#_Toc172624472"^^xsd:anyURI .

C1901A00006:719 a legcons:Item,
        skos:Concept,
        dcat:Resource ;
    rdfs:label "Item I719"@en-AU ;
    rdfs:comment "153 ZMC  Goods wholly obtained in Korea or in Korea and Australia - GraphNodeID: I719"@en-AU ;
    skos:definition "153 ZMC  Goods wholly obtained in Korea or in Korea and Australia"@en-AU ;
    skos:narrower C1901A00006:718 ;
    skos:prefLabel "Item I719"@en-AU ;
    dcat:accessURL "https://www.legislation.gov.au/C1901A00006/2024-07-01/2024-07-01/text/original/epub/OEBPS/document_2/document_2.html#_Toc172624474"^^xsd:anyURI .

C1901A00006:72 a legcons:Item,
        skos:Concept,
        dcat:Resource ;
    rdfs:label "Item I72"@en-AU ;
    rdfs:comment "62  Ships to come quickly to place of unlading - GraphNodeID: I72"@en-AU ;
    skos:definition "62  Ships to come quickly to place of unlading"@en-AU ;
    skos:narrower C1901A00006:65 ;
    skos:prefLabel "Item I72"@en-AU ;
    dcat:accessURL "https://www.legislation.gov.au/C1901A00006/2024-07-01/2024-07-01/text/original/epub/OEBPS/document_1/document_1.html#_Toc172623046"^^xsd:anyURI .

C1901A00006:721 a legcons:Item,
        skos:Concept,
        dcat:Resource ;
    rdfs:label "Item I721"@en-AU ;
    rdfs:comment "153 ZMD  Goods produced in Korea or in Korea and Australia from originating materials - GraphNodeID: I721"@en-AU ;
    skos:definition "153 ZMD  Goods produced in Korea or in Korea and Australia from originating materials"@en-AU ;
    skos:narrower C1901A00006:720 ;
    skos:prefLabel "Item I721"@en-AU ;
    dcat:accessURL "https://www.legislation.gov.au/C1901A00006/2024-07-01/2024-07-01/text/original/epub/OEBPS/document_2/document_2.html#_Toc172624476"^^xsd:anyURI .

C1901A00006:723 a legcons:Item,
        skos:Concept,
        dcat:Resource ;
    rdfs:label "Item I723"@en-AU ;
    rdfs:comment "153 ZME  Goods produced in Korea or in Korea and Australia from non originating materials - GraphNodeID: I723"@en-AU ;
    skos:definition "153 ZME  Goods produced in Korea or in Korea and Australia from non originating materials"@en-AU ;
    skos:narrower C1901A00006:722 ;
    skos:prefLabel "Item I723"@en-AU ;
    dcat:accessURL "https://www.legislation.gov.au/C1901A00006/2024-07-01/2024-07-01/text/original/epub/OEBPS/document_2/document_2.html#_Toc172624478"^^xsd:anyURI .

C1901A00006:724 a legcons:Item,
        skos:Concept,
        dcat:Resource ;
    rdfs:label "Item I724"@en-AU ;
    rdfs:comment "153 ZMF  Packaging materials and containers - GraphNodeID: I724"@en-AU ;
    skos:definition "153 ZMF  Packaging materials and containers"@en-AU ;
    skos:narrower C1901A00006:722 ;
    skos:prefLabel "Item I724"@en-AU ;
    dcat:accessURL "https://www.legislation.gov.au/C1901A00006/2024-07-01/2024-07-01/text/original/epub/OEBPS/document_2/document_2.html#_Toc172624479"^^xsd:anyURI .

C1901A00006:726 a legcons:Item,
        skos:Concept,
        dcat:Resource ;
    rdfs:label "Item I726"@en-AU ;
    rdfs:comment "153 ZMG  Non qualifying operations - GraphNodeID: I726"@en-AU ;
    skos:definition "153 ZMG  Non qualifying operations"@en-AU ;
    skos:narrower C1901A00006:725 ;
    skos:prefLabel "Item I726"@en-AU ;
    dcat:accessURL "https://www.legislation.gov.au/C1901A00006/2024-07-01/2024-07-01/text/original/epub/OEBPS/document_2/document_2.html#_Toc172624481"^^xsd:anyURI .

C1901A00006:728 a legcons:Item,
        skos:Concept,
        dcat:Resource ;
    rdfs:label "Item I728"@en-AU ;
    rdfs:comment "153 ZMH  Consignment - GraphNodeID: I728"@en-AU ;
    skos:definition "153 ZMH  Consignment"@en-AU ;
    skos:narrower C1901A00006:727 ;
    skos:prefLabel "Item I728"@en-AU ;
    dcat:accessURL "https://www.legislation.gov.au/C1901A00006/2024-07-01/2024-07-01/text/original/epub/OEBPS/document_2/document_2.html#_Toc172624483"^^xsd:anyURI .

C1901A00006:729 a legcons:Item,
        skos:Concept,
        dcat:Resource ;
    rdfs:label "Item I729"@en-AU ;
    rdfs:comment "153 ZMI  Outward processing zones on the Korean Peninsula - GraphNodeID: I729"@en-AU ;
    skos:definition "153 ZMI  Outward processing zones on the Korean Peninsula"@en-AU ;
    skos:narrower C1901A00006:727 ;
    skos:prefLabel "Item I729"@en-AU ;
    dcat:accessURL "https://www.legislation.gov.au/C1901A00006/2024-07-01/2024-07-01/text/original/epub/OEBPS/document_2/document_2.html#_Toc172624484"^^xsd:anyURI .

C1901A00006:73 a legcons:Item,
        skos:Concept,
        dcat:Resource ;
    rdfs:label "Item I73"@en-AU ;
    rdfs:comment "63  Ship or aircraft not to be moved without authority - GraphNodeID: I73"@en-AU ;
    skos:definition "63  Ship or aircraft not to be moved without authority"@en-AU ;
    skos:narrower C1901A00006:65 ;
    skos:prefLabel "Item I73"@en-AU ;
    dcat:accessURL "https://www.legislation.gov.au/C1901A00006/2024-07-01/2024-07-01/text/original/epub/OEBPS/document_1/document_1.html#_Toc172623047"^^xsd:anyURI .

C1901A00006:730 a legcons:Item,
        skos:Concept,
        dcat:Resource ;
    rdfs:label "Item I730"@en-AU ;
    rdfs:comment "153 ZMJ  Regulations - GraphNodeID: I730"@en-AU ;
    skos:definition "153 ZMJ  Regulations"@en-AU ;
    skos:narrower C1901A00006:727 ;
    skos:prefLabel "Item I730"@en-AU ;
    dcat:accessURL "https://www.legislation.gov.au/C1901A00006/2024-07-01/2024-07-01/text/original/epub/OEBPS/document_2/document_2.html#_Toc172624485"^^xsd:anyURI .

C1901A00006:733 a legcons:Item,
        skos:Concept,
        dcat:Resource ;
    rdfs:label "Item I733"@en-AU ;
    rdfs:comment "153 ZMK  Simplified outline of this Division - GraphNodeID: I733"@en-AU ;
    skos:definition "153 ZMK  Simplified outline of this Division"@en-AU ;
    skos:narrower C1901A00006:732 ;
    skos:prefLabel "Item I733"@en-AU ;
    dcat:accessURL "https://www.legislation.gov.au/C1901A00006/2024-07-01/2024-07-01/text/original/epub/OEBPS/document_2/document_2.html#_Toc172624488"^^xsd:anyURI .

C1901A00006:734 a legcons:Item,
        skos:Concept,
        dcat:Resource ;
    rdfs:label "Item I734"@en-AU ;
    rdfs:comment "153 ZML  Interpretation - GraphNodeID: I734"@en-AU ;
    skos:definition "153 ZML  Interpretation"@en-AU ;
    skos:narrower C1901A00006:732 ;
    skos:prefLabel "Item I734"@en-AU ;
    dcat:accessURL "https://www.legislation.gov.au/C1901A00006/2024-07-01/2024-07-01/text/original/epub/OEBPS/document_2/document_2.html#_Toc172624489"^^xsd:anyURI .

C1901A00006:736 a legcons:Item,
        skos:Concept,
        dcat:Resource ;
    rdfs:label "Item I736"@en-AU ;
    rdfs:comment "153 ZMM  Goods wholly obtained or produced in India or in India and Australia - GraphNodeID: I736"@en-AU ;
    skos:definition "153 ZMM  Goods wholly obtained or produced in India or in India and Australia"@en-AU ;
    skos:narrower C1901A00006:735 ;
    skos:prefLabel "Item I736"@en-AU ;
    dcat:accessURL "https://www.legislation.gov.au/C1901A00006/2024-07-01/2024-07-01/text/original/epub/OEBPS/document_2/document_2.html#_Toc172624491"^^xsd:anyURI .

C1901A00006:738 a legcons:Item,
        skos:Concept,
        dcat:Resource ;
    rdfs:label "Item I738"@en-AU ;
    rdfs:comment "153 ZMN  Goods produced in India or in India and Australia from non originating materials - GraphNodeID: I738"@en-AU ;
    skos:definition "153 ZMN  Goods produced in India or in India and Australia from non originating materials"@en-AU ;
    skos:narrower C1901A00006:737 ;
    skos:prefLabel "Item I738"@en-AU ;
    dcat:accessURL "https://www.legislation.gov.au/C1901A00006/2024-07-01/2024-07-01/text/original/epub/OEBPS/document_2/document_2.html#_Toc172624493"^^xsd:anyURI .

C1901A00006:739 a legcons:Item,
        skos:Concept,
        dcat:Resource ;
    rdfs:label "Item I739"@en-AU ;
    rdfs:comment "153 ZMO  Non qualifying operations - GraphNodeID: I739"@en-AU ;
    skos:definition "153 ZMO  Non qualifying operations"@en-AU ;
    skos:narrower C1901A00006:737 ;
    skos:prefLabel "Item I739"@en-AU ;
    dcat:accessURL "https://www.legislation.gov.au/C1901A00006/2024-07-01/2024-07-01/text/original/epub/OEBPS/document_2/document_2.html#_Toc172624494"^^xsd:anyURI .

C1901A00006:741 a legcons:Item,
        skos:Concept,
        dcat:Resource ;
    rdfs:label "Item I741"@en-AU ;
    rdfs:comment "153 ZMP  Packaging materials and containers - GraphNodeID: I741"@en-AU ;
    skos:definition "153 ZMP  Packaging materials and containers"@en-AU ;
    skos:narrower C1901A00006:740 ;
    skos:prefLabel "Item I741"@en-AU ;
    dcat:accessURL "https://www.legislation.gov.au/C1901A00006/2024-07-01/2024-07-01/text/original/epub/OEBPS/document_2/document_2.html#_Toc172624496"^^xsd:anyURI .

C1901A00006:743 a legcons:Item,
        skos:Concept,
        dcat:Resource ;
    rdfs:label "Item I743"@en-AU ;
    rdfs:comment "153 ZMQ  Consignment - GraphNodeID: I743"@en-AU ;
    skos:definition "153 ZMQ  Consignment"@en-AU ;
    skos:narrower C1901A00006:742 ;
    skos:prefLabel "Item I743"@en-AU ;
    dcat:accessURL "https://www.legislation.gov.au/C1901A00006/2024-07-01/2024-07-01/text/original/epub/OEBPS/document_2/document_2.html#_Toc172624498"^^xsd:anyURI .

C1901A00006:745 a legcons:Item,
        skos:Concept,
        dcat:Resource ;
    rdfs:label "Item I745"@en-AU ;
    rdfs:comment "153 ZMR  Regulations - GraphNodeID: I745"@en-AU ;
    skos:definition "153 ZMR  Regulations"@en-AU ;
    skos:narrower C1901A00006:744 ;
    skos:prefLabel "Item I745"@en-AU ;
    dcat:accessURL "https://www.legislation.gov.au/C1901A00006/2024-07-01/2024-07-01/text/original/epub/OEBPS/document_2/document_2.html#_Toc172624500"^^xsd:anyURI .

C1901A00006:748 a legcons:Item,
        skos:Concept,
        dcat:Resource ;
    rdfs:label "Item I748"@en-AU ;
    rdfs:comment "153 ZNA  Simplified outline of this Division - GraphNodeID: I748"@en-AU ;
    skos:definition "153 ZNA  Simplified outline of this Division"@en-AU ;
    skos:narrower C1901A00006:747 ;
    skos:prefLabel "Item I748"@en-AU ;
    dcat:accessURL "https://www.legislation.gov.au/C1901A00006/2024-07-01/2024-07-01/text/original/epub/OEBPS/document_2/document_2.html#_Toc172624503"^^xsd:anyURI .

C1901A00006:749 a legcons:Item,
        skos:Concept,
        dcat:Resource ;
    rdfs:label "Item I749"@en-AU ;
    rdfs:comment "153 ZNB  Interpretation - GraphNodeID: I749"@en-AU ;
    skos:definition "153 ZNB  Interpretation"@en-AU ;
    skos:narrower C1901A00006:747 ;
    skos:prefLabel "Item I749"@en-AU ;
    dcat:accessURL "https://www.legislation.gov.au/C1901A00006/2024-07-01/2024-07-01/text/original/epub/OEBPS/document_2/document_2.html#_Toc172624504"^^xsd:anyURI .

C1901A00006:751 a legcons:Item,
        skos:Concept,
        dcat:Resource ;
    rdfs:label "Item I751"@en-AU ;
    rdfs:comment "153 ZNC  Goods wholly obtained in Japan - GraphNodeID: I751"@en-AU ;
    skos:definition "153 ZNC  Goods wholly obtained in Japan"@en-AU ;
    skos:narrower C1901A00006:750 ;
    skos:prefLabel "Item I751"@en-AU ;
    dcat:accessURL "https://www.legislation.gov.au/C1901A00006/2024-07-01/2024-07-01/text/original/epub/OEBPS/document_2/document_2.html#_Toc172624506"^^xsd:anyURI .

C1901A00006:753 a legcons:Item,
        skos:Concept,
        dcat:Resource ;
    rdfs:label "Item I753"@en-AU ;
    rdfs:comment "153 ZND  Goods produced in Japan from originating materials - GraphNodeID: I753"@en-AU ;
    skos:definition "153 ZND  Goods produced in Japan from originating materials"@en-AU ;
    skos:narrower C1901A00006:752 ;
    skos:prefLabel "Item I753"@en-AU ;
    dcat:accessURL "https://www.legislation.gov.au/C1901A00006/2024-07-01/2024-07-01/text/original/epub/OEBPS/document_2/document_2.html#_Toc172624508"^^xsd:anyURI .

C1901A00006:755 a legcons:Item,
        skos:Concept,
        dcat:Resource ;
    rdfs:label "Item I755"@en-AU ;
    rdfs:comment "153 ZNE  Goods produced in Japan or in Japan and Australia from non originating materials - GraphNodeID: I755"@en-AU ;
    skos:definition "153 ZNE  Goods produced in Japan or in Japan and Australia from non originating materials"@en-AU ;
    skos:narrower C1901A00006:754 ;
    skos:prefLabel "Item I755"@en-AU ;
    dcat:accessURL "https://www.legislation.gov.au/C1901A00006/2024-07-01/2024-07-01/text/original/epub/OEBPS/document_2/document_2.html#_Toc172624510"^^xsd:anyURI .

C1901A00006:756 a legcons:Item,
        skos:Concept,
        dcat:Resource ;
    rdfs:label "Item I756"@en-AU ;
    rdfs:comment "153 ZNF  Packaging materials and containers - GraphNodeID: I756"@en-AU ;
    skos:definition "153 ZNF  Packaging materials and containers"@en-AU ;
    skos:narrower C1901A00006:754 ;
    skos:prefLabel "Item I756"@en-AU ;
    dcat:accessURL "https://www.legislation.gov.au/C1901A00006/2024-07-01/2024-07-01/text/original/epub/OEBPS/document_2/document_2.html#_Toc172624511"^^xsd:anyURI .

C1901A00006:757 a legcons:Item,
        skos:Concept,
        dcat:Resource ;
    rdfs:label "Item I757"@en-AU ;
    rdfs:comment "153 ZNG  Non qualifying operations - GraphNodeID: I757"@en-AU ;
    skos:definition "153 ZNG  Non qualifying operations"@en-AU ;
    skos:narrower C1901A00006:754 ;
    skos:prefLabel "Item I757"@en-AU ;
    dcat:accessURL "https://www.legislation.gov.au/C1901A00006/2024-07-01/2024-07-01/text/original/epub/OEBPS/document_2/document_2.html#_Toc172624512"^^xsd:anyURI .

C1901A00006:759 a legcons:Item,
        skos:Concept,
        dcat:Resource ;
    rdfs:label "Item I759"@en-AU ;
    rdfs:comment "153 ZNH  Consignment - GraphNodeID: I759"@en-AU ;
    skos:definition "153 ZNH  Consignment"@en-AU ;
    skos:narrower C1901A00006:758 ;
    skos:prefLabel "Item I759"@en-AU ;
    dcat:accessURL "https://www.legislation.gov.au/C1901A00006/2024-07-01/2024-07-01/text/original/epub/OEBPS/document_2/document_2.html#_Toc172624514"^^xsd:anyURI .

C1901A00006:76 a legcons:Item,
        skos:Concept,
        dcat:Resource ;
    rdfs:label "Item I76"@en-AU ;
    rdfs:comment "63 A  Definitions - GraphNodeID: I76"@en-AU ;
    skos:definition "63 A  Definitions"@en-AU ;
    skos:narrower C1901A00006:75 ;
    skos:prefLabel "Item I76"@en-AU ;
    dcat:accessURL "https://www.legislation.gov.au/C1901A00006/2024-07-01/2024-07-01/text/original/epub/OEBPS/document_1/document_1.html#_Toc172623050"^^xsd:anyURI .

C1901A00006:761 a legcons:Item,
        skos:Concept,
        dcat:Resource ;
    rdfs:label "Item I761"@en-AU ;
    rdfs:comment "153 ZNI  Regulations - GraphNodeID: I761"@en-AU ;
    skos:definition "153 ZNI  Regulations"@en-AU ;
    skos:narrower C1901A00006:760 ;
    skos:prefLabel "Item I761"@en-AU ;
    dcat:accessURL "https://www.legislation.gov.au/C1901A00006/2024-07-01/2024-07-01/text/original/epub/OEBPS/document_2/document_2.html#_Toc172624516"^^xsd:anyURI .

C1901A00006:764 a legcons:Item,
        skos:Concept,
        dcat:Resource ;
    rdfs:label "Item I764"@en-AU ;
    rdfs:comment "153 ZOA  Simplified outline of this Division - GraphNodeID: I764"@en-AU ;
    skos:definition "153 ZOA  Simplified outline of this Division"@en-AU ;
    skos:narrower C1901A00006:763 ;
    skos:prefLabel "Item I764"@en-AU ;
    dcat:accessURL "https://www.legislation.gov.au/C1901A00006/2024-07-01/2024-07-01/text/original/epub/OEBPS/document_2/document_2.html#_Toc172624519"^^xsd:anyURI .

C1901A00006:765 a legcons:Item,
        skos:Concept,
        dcat:Resource ;
    rdfs:label "Item I765"@en-AU ;
    rdfs:comment "153 ZOB  Interpretation - GraphNodeID: I765"@en-AU ;
    skos:definition "153 ZOB  Interpretation"@en-AU ;
    skos:narrower C1901A00006:763 ;
    skos:prefLabel "Item I765"@en-AU ;
    dcat:accessURL "https://www.legislation.gov.au/C1901A00006/2024-07-01/2024-07-01/text/original/epub/OEBPS/document_2/document_2.html#_Toc172624520"^^xsd:anyURI .

C1901A00006:767 a legcons:Item,
        skos:Concept,
        dcat:Resource ;
    rdfs:label "Item I767"@en-AU ;
    rdfs:comment "153 ZOC  Goods wholly obtained or produced in the territory of China - GraphNodeID: I767"@en-AU ;
    skos:definition "153 ZOC  Goods wholly obtained or produced in the territory of China"@en-AU ;
    skos:narrower C1901A00006:766 ;
    skos:prefLabel "Item I767"@en-AU ;
    dcat:accessURL "https://www.legislation.gov.au/C1901A00006/2024-07-01/2024-07-01/text/original/epub/OEBPS/document_2/document_2.html#_Toc172624522"^^xsd:anyURI .

C1901A00006:769 a legcons:Item,
        skos:Concept,
        dcat:Resource ;
    rdfs:label "Item I769"@en-AU ;
    rdfs:comment "153 ZOD  Goods produced in China or in China and Australia from originating materials - GraphNodeID: I769"@en-AU ;
    skos:definition "153 ZOD  Goods produced in China or in China and Australia from originating materials"@en-AU ;
    skos:narrower C1901A00006:768 ;
    skos:prefLabel "Item I769"@en-AU ;
    dcat:accessURL "https://www.legislation.gov.au/C1901A00006/2024-07-01/2024-07-01/text/original/epub/OEBPS/document_2/document_2.html#_Toc172624524"^^xsd:anyURI .

C1901A00006:77 a legcons:Item,
        skos:Concept,
        dcat:Resource ;
    rdfs:label "Item I77"@en-AU ;
    rdfs:comment "64  Impending arrival report - GraphNodeID: I77"@en-AU ;
    skos:definition "64  Impending arrival report"@en-AU ;
    skos:narrower C1901A00006:75 ;
    skos:prefLabel "Item I77"@en-AU ;
    dcat:accessURL "https://www.legislation.gov.au/C1901A00006/2024-07-01/2024-07-01/text/original/epub/OEBPS/document_1/document_1.html#_Toc172623051"^^xsd:anyURI .

C1901A00006:771 a legcons:Item,
        skos:Concept,
        dcat:Resource ;
    rdfs:label "Item I771"@en-AU ;
    rdfs:comment "153 ZOE  Goods produced in China or in China and Australia from non originating materials - GraphNodeID: I771"@en-AU ;
    skos:definition "153 ZOE  Goods produced in China or in China and Australia from non originating materials"@en-AU ;
    skos:narrower C1901A00006:770 ;
    skos:prefLabel "Item I771"@en-AU ;
    dcat:accessURL "https://www.legislation.gov.au/C1901A00006/2024-07-01/2024-07-01/text/original/epub/OEBPS/document_2/document_2.html#_Toc172624526"^^xsd:anyURI .

C1901A00006:772 a legcons:Item,
        skos:Concept,
        dcat:Resource ;
    rdfs:label "Item I772"@en-AU ;
    rdfs:comment "153 ZOF  Packaging materials and containers - GraphNodeID: I772"@en-AU ;
    skos:definition "153 ZOF  Packaging materials and containers"@en-AU ;
    skos:narrower C1901A00006:770 ;
    skos:prefLabel "Item I772"@en-AU ;
    dcat:accessURL "https://www.legislation.gov.au/C1901A00006/2024-07-01/2024-07-01/text/original/epub/OEBPS/document_2/document_2.html#_Toc172624527"^^xsd:anyURI .

C1901A00006:774 a legcons:Item,
        skos:Concept,
        dcat:Resource ;
    rdfs:label "Item I774"@en-AU ;
    rdfs:comment "153 ZOG  Goods that are accessories spare parts or tools - GraphNodeID: I774"@en-AU ;
    skos:definition "153 ZOG  Goods that are accessories spare parts or tools"@en-AU ;
    skos:narrower C1901A00006:773 ;
    skos:prefLabel "Item I774"@en-AU ;
    dcat:accessURL "https://www.legislation.gov.au/C1901A00006/2024-07-01/2024-07-01/text/original/epub/OEBPS/document_2/document_2.html#_Toc172624529"^^xsd:anyURI .

C1901A00006:776 a legcons:Item,
        skos:Concept,
        dcat:Resource ;
    rdfs:label "Item I776"@en-AU ;
    rdfs:comment "153 ZOH  Non qualifying operations - GraphNodeID: I776"@en-AU ;
    skos:definition "153 ZOH  Non qualifying operations"@en-AU ;
    skos:narrower C1901A00006:775 ;
    skos:prefLabel "Item I776"@en-AU ;
    dcat:accessURL "https://www.legislation.gov.au/C1901A00006/2024-07-01/2024-07-01/text/original/epub/OEBPS/document_2/document_2.html#_Toc172624531"^^xsd:anyURI .

C1901A00006:778 a legcons:Item,
        skos:Concept,
        dcat:Resource ;
    rdfs:label "Item I778"@en-AU ;
    rdfs:comment "153 ZOI  Consignment - GraphNodeID: I778"@en-AU ;
    skos:definition "153 ZOI  Consignment"@en-AU ;
    skos:narrower C1901A00006:777 ;
    skos:prefLabel "Item I778"@en-AU ;
    dcat:accessURL "https://www.legislation.gov.au/C1901A00006/2024-07-01/2024-07-01/text/original/epub/OEBPS/document_2/document_2.html#_Toc172624533"^^xsd:anyURI .

C1901A00006:78 a legcons:Item,
        skos:Concept,
        dcat:Resource ;
    rdfs:label "Item I78"@en-AU ;
    rdfs:comment "64 AA  Arrival report - GraphNodeID: I78"@en-AU ;
    skos:definition "64 AA  Arrival report"@en-AU ;
    skos:narrower C1901A00006:75 ;
    skos:prefLabel "Item I78"@en-AU ;
    dcat:accessURL "https://www.legislation.gov.au/C1901A00006/2024-07-01/2024-07-01/text/original/epub/OEBPS/document_1/document_1.html#_Toc172623052"^^xsd:anyURI .

C1901A00006:780 a legcons:Item,
        skos:Concept,
        dcat:Resource ;
    rdfs:label "Item I780"@en-AU ;
    rdfs:comment "153 ZOJ  Regulations - GraphNodeID: I780"@en-AU ;
    skos:definition "153 ZOJ  Regulations"@en-AU ;
    skos:narrower C1901A00006:779 ;
    skos:prefLabel "Item I780"@en-AU ;
    dcat:accessURL "https://www.legislation.gov.au/C1901A00006/2024-07-01/2024-07-01/text/original/epub/OEBPS/document_2/document_2.html#_Toc172624535"^^xsd:anyURI .

C1901A00006:783 a legcons:Item,
        skos:Concept,
        dcat:Resource ;
    rdfs:label "Item I783"@en-AU ;
    rdfs:comment "153 ZPA  Simplified outline of this Division - GraphNodeID: I783"@en-AU ;
    skos:definition "153 ZPA  Simplified outline of this Division"@en-AU ;
    skos:narrower C1901A00006:782 ;
    skos:prefLabel "Item I783"@en-AU ;
    dcat:accessURL "https://www.legislation.gov.au/C1901A00006/2024-07-01/2024-07-01/text/original/epub/OEBPS/document_2/document_2.html#_Toc172624538"^^xsd:anyURI .

C1901A00006:784 a legcons:Item,
        skos:Concept,
        dcat:Resource ;
    rdfs:label "Item I784"@en-AU ;
    rdfs:comment "153 ZPB  Interpretation - GraphNodeID: I784"@en-AU ;
    skos:definition "153 ZPB  Interpretation"@en-AU ;
    skos:narrower C1901A00006:782 ;
    skos:prefLabel "Item I784"@en-AU ;
    dcat:accessURL "https://www.legislation.gov.au/C1901A00006/2024-07-01/2024-07-01/text/original/epub/OEBPS/document_2/document_2.html#_Toc172624539"^^xsd:anyURI .

C1901A00006:786 a legcons:Item,
        skos:Concept,
        dcat:Resource ;
    rdfs:label "Item I786"@en-AU ;
    rdfs:comment "153 ZPC  Goods wholly obtained or produced entirely in Hong Kong China or in Hong Kong China and Australia - GraphNodeID: I786"@en-AU ;
    skos:definition "153 ZPC  Goods wholly obtained or produced entirely in Hong Kong China or in Hong Kong China and Australia"@en-AU ;
    skos:narrower C1901A00006:785 ;
    skos:prefLabel "Item I786"@en-AU ;
    dcat:accessURL "https://www.legislation.gov.au/C1901A00006/2024-07-01/2024-07-01/text/original/epub/OEBPS/document_2/document_2.html#_Toc172624541"^^xsd:anyURI .

C1901A00006:788 a legcons:Item,
        skos:Concept,
        dcat:Resource ;
    rdfs:label "Item I788"@en-AU ;
    rdfs:comment "153 ZPD  Goods produced in Hong Kong China or in Hong Kong China and Australia from originating materials - GraphNodeID: I788"@en-AU ;
    skos:definition "153 ZPD  Goods produced in Hong Kong China or in Hong Kong China and Australia from originating materials"@en-AU ;
    skos:narrower C1901A00006:787 ;
    skos:prefLabel "Item I788"@en-AU ;
    dcat:accessURL "https://www.legislation.gov.au/C1901A00006/2024-07-01/2024-07-01/text/original/epub/OEBPS/document_2/document_2.html#_Toc172624543"^^xsd:anyURI .

C1901A00006:79 a legcons:Item,
        skos:Concept,
        dcat:Resource ;
    rdfs:label "Item I79"@en-AU ;
    rdfs:comment "64 AAA  Report of stores and prohibited goods - GraphNodeID: I79"@en-AU ;
    skos:definition "64 AAA  Report of stores and prohibited goods"@en-AU ;
    skos:narrower C1901A00006:75 ;
    skos:prefLabel "Item I79"@en-AU ;
    dcat:accessURL "https://www.legislation.gov.au/C1901A00006/2024-07-01/2024-07-01/text/original/epub/OEBPS/document_1/document_1.html#_Toc172623053"^^xsd:anyURI .

C1901A00006:790 a legcons:Item,
        skos:Concept,
        dcat:Resource ;
    rdfs:label "Item I790"@en-AU ;
    rdfs:comment "153 ZPE  Goods produced in Hong Kong China or in Hong Kong China and Australia from non originating materials - GraphNodeID: I790"@en-AU ;
    skos:definition "153 ZPE  Goods produced in Hong Kong China or in Hong Kong China and Australia from non originating materials"@en-AU ;
    skos:narrower C1901A00006:789 ;
    skos:prefLabel "Item I790"@en-AU ;
    dcat:accessURL "https://www.legislation.gov.au/C1901A00006/2024-07-01/2024-07-01/text/original/epub/OEBPS/document_2/document_2.html#_Toc172624545"^^xsd:anyURI .

C1901A00006:791 a legcons:Item,
        skos:Concept,
        dcat:Resource ;
    rdfs:label "Item I791"@en-AU ;
    rdfs:comment "153 ZPF  Packaging materials and containers - GraphNodeID: I791"@en-AU ;
    skos:definition "153 ZPF  Packaging materials and containers"@en-AU ;
    skos:narrower C1901A00006:789 ;
    skos:prefLabel "Item I791"@en-AU ;
    dcat:accessURL "https://www.legislation.gov.au/C1901A00006/2024-07-01/2024-07-01/text/original/epub/OEBPS/document_2/document_2.html#_Toc172624546"^^xsd:anyURI .

C1901A00006:793 a legcons:Item,
        skos:Concept,
        dcat:Resource ;
    rdfs:label "Item I793"@en-AU ;
    rdfs:comment "153 ZPG  Goods that are accessories spare parts tools or instructional or other information materials - GraphNodeID: I793"@en-AU ;
    skos:definition "153 ZPG  Goods that are accessories spare parts tools or instructional or other information materials"@en-AU ;
    skos:narrower C1901A00006:792 ;
    skos:prefLabel "Item I793"@en-AU ;
    dcat:accessURL "https://www.legislation.gov.au/C1901A00006/2024-07-01/2024-07-01/text/original/epub/OEBPS/document_2/document_2.html#_Toc172624548"^^xsd:anyURI .

C1901A00006:795 a legcons:Item,
        skos:Concept,
        dcat:Resource ;
    rdfs:label "Item I795"@en-AU ;
    rdfs:comment "153 ZPH  Consignment - GraphNodeID: I795"@en-AU ;
    skos:definition "153 ZPH  Consignment"@en-AU ;
    skos:narrower C1901A00006:794 ;
    skos:prefLabel "Item I795"@en-AU ;
    dcat:accessURL "https://www.legislation.gov.au/C1901A00006/2024-07-01/2024-07-01/text/original/epub/OEBPS/document_2/document_2.html#_Toc172624550"^^xsd:anyURI .

C1901A00006:797 a legcons:Item,
        skos:Concept,
        dcat:Resource ;
    rdfs:label "Item I797"@en-AU ;
    rdfs:comment "153 ZPI  Regulations - GraphNodeID: I797"@en-AU ;
    skos:definition "153 ZPI  Regulations"@en-AU ;
    skos:narrower C1901A00006:796 ;
    skos:prefLabel "Item I797"@en-AU ;
    dcat:accessURL "https://www.legislation.gov.au/C1901A00006/2024-07-01/2024-07-01/text/original/epub/OEBPS/document_2/document_2.html#_Toc172624552"^^xsd:anyURI .

C1901A00006:8 a legcons:Item,
        skos:Concept,
        dcat:Resource ;
    rdfs:label "Item I8"@en-AU ;
    rdfs:comment "4 AB  Compensation for acquisition of property - GraphNodeID: I8"@en-AU ;
    skos:definition "4 AB  Compensation for acquisition of property"@en-AU ;
    skos:narrower C1901A00006:2 ;
    skos:prefLabel "Item I8"@en-AU ;
    dcat:accessURL "https://www.legislation.gov.au/C1901A00006/2024-07-01/2024-07-01/text/original/epub/OEBPS/document_1/document_1.html#_Toc172622982"^^xsd:anyURI .

C1901A00006:80 a legcons:Item,
        skos:Concept,
        dcat:Resource ;
    rdfs:label "Item I80"@en-AU ;
    rdfs:comment "64 AAB  Notifying Department of particulars of cargo reporters - GraphNodeID: I80"@en-AU ;
    skos:definition "64 AAB  Notifying Department of particulars of cargo reporters"@en-AU ;
    skos:narrower C1901A00006:75 ;
    skos:prefLabel "Item I80"@en-AU ;
    dcat:accessURL "https://www.legislation.gov.au/C1901A00006/2024-07-01/2024-07-01/text/original/epub/OEBPS/document_1/document_1.html#_Toc172623054"^^xsd:anyURI .

C1901A00006:800 a legcons:Item,
        skos:Concept,
        dcat:Resource ;
    rdfs:label "Item I800"@en-AU ;
    rdfs:comment "153 ZQA  Simplified outline of this Division - GraphNodeID: I800"@en-AU ;
    skos:definition "153 ZQA  Simplified outline of this Division"@en-AU ;
    skos:narrower C1901A00006:799 ;
    skos:prefLabel "Item I800"@en-AU ;
    dcat:accessURL "https://www.legislation.gov.au/C1901A00006/2024-07-01/2024-07-01/text/original/epub/OEBPS/document_2/document_2.html#_Toc172624555"^^xsd:anyURI .

C1901A00006:801 a legcons:Item,
        skos:Concept,
        dcat:Resource ;
    rdfs:label "Item I801"@en-AU ;
    rdfs:comment "153 ZQB  Interpretation - GraphNodeID: I801"@en-AU ;
    skos:definition "153 ZQB  Interpretation"@en-AU ;
    skos:narrower C1901A00006:799 ;
    skos:prefLabel "Item I801"@en-AU ;
    dcat:accessURL "https://www.legislation.gov.au/C1901A00006/2024-07-01/2024-07-01/text/original/epub/OEBPS/document_2/document_2.html#_Toc172624556"^^xsd:anyURI .

C1901A00006:803 a legcons:Item,
        skos:Concept,
        dcat:Resource ;
    rdfs:label "Item I803"@en-AU ;
    rdfs:comment "153 ZQC  Goods wholly obtained or produced in a Party - GraphNodeID: I803"@en-AU ;
    skos:definition "153 ZQC  Goods wholly obtained or produced in a Party"@en-AU ;
    skos:narrower C1901A00006:802 ;
    skos:prefLabel "Item I803"@en-AU ;
    dcat:accessURL "https://www.legislation.gov.au/C1901A00006/2024-07-01/2024-07-01/text/original/epub/OEBPS/document_2/document_2.html#_Toc172624558"^^xsd:anyURI .

C1901A00006:805 a legcons:Item,
        skos:Concept,
        dcat:Resource ;
    rdfs:label "Item I805"@en-AU ;
    rdfs:comment "153 ZQD  Goods produced from originating materials - GraphNodeID: I805"@en-AU ;
    skos:definition "153 ZQD  Goods produced from originating materials"@en-AU ;
    skos:narrower C1901A00006:804 ;
    skos:prefLabel "Item I805"@en-AU ;
    dcat:accessURL "https://www.legislation.gov.au/C1901A00006/2024-07-01/2024-07-01/text/original/epub/OEBPS/document_2/document_2.html#_Toc172624560"^^xsd:anyURI .

C1901A00006:807 a legcons:Item,
        skos:Concept,
        dcat:Resource ;
    rdfs:label "Item I807"@en-AU ;
    rdfs:comment "153 ZQE  Goods produced from non originating materials - GraphNodeID: I807"@en-AU ;
    skos:definition "153 ZQE  Goods produced from non originating materials"@en-AU ;
    skos:narrower C1901A00006:806 ;
    skos:prefLabel "Item I807"@en-AU ;
    dcat:accessURL "https://www.legislation.gov.au/C1901A00006/2024-07-01/2024-07-01/text/original/epub/OEBPS/document_2/document_2.html#_Toc172624562"^^xsd:anyURI .

C1901A00006:808 a legcons:Item,
        skos:Concept,
        dcat:Resource ;
    rdfs:label "Item I808"@en-AU ;
    rdfs:comment "153 ZQF  Packaging materials and containers - GraphNodeID: I808"@en-AU ;
    skos:definition "153 ZQF  Packaging materials and containers"@en-AU ;
    skos:narrower C1901A00006:806 ;
    skos:prefLabel "Item I808"@en-AU ;
    dcat:accessURL "https://www.legislation.gov.au/C1901A00006/2024-07-01/2024-07-01/text/original/epub/OEBPS/document_2/document_2.html#_Toc172624563"^^xsd:anyURI .

C1901A00006:809 a legcons:Item,
        skos:Concept,
        dcat:Resource ;
    rdfs:label "Item I809"@en-AU ;
    rdfs:comment "153 ZQG  Accessories spare parts tools or instructional or other information materials - GraphNodeID: I809"@en-AU ;
    skos:definition "153 ZQG  Accessories spare parts tools or instructional or other information materials"@en-AU ;
    skos:narrower C1901A00006:806 ;
    skos:prefLabel "Item I809"@en-AU ;
    dcat:accessURL "https://www.legislation.gov.au/C1901A00006/2024-07-01/2024-07-01/text/original/epub/OEBPS/document_2/document_2.html#_Toc172624564"^^xsd:anyURI .

C1901A00006:81 a legcons:Item,
        skos:Concept,
        dcat:Resource ;
    rdfs:label "Item I81"@en-AU ;
    rdfs:comment "64 AAC  Report to Department of persons engaged to unload cargo - GraphNodeID: I81"@en-AU ;
    skos:definition "64 AAC  Report to Department of persons engaged to unload cargo"@en-AU ;
    skos:narrower C1901A00006:75 ;
    skos:prefLabel "Item I81"@en-AU ;
    dcat:accessURL "https://www.legislation.gov.au/C1901A00006/2024-07-01/2024-07-01/text/original/epub/OEBPS/document_1/document_1.html#_Toc172623055"^^xsd:anyURI .

C1901A00006:810 a legcons:Item,
        skos:Concept,
        dcat:Resource ;
    rdfs:label "Item I810"@en-AU ;
    rdfs:comment "153 ZQH  Non qualifying operations or processes - GraphNodeID: I810"@en-AU ;
    skos:definition "153 ZQH  Non qualifying operations or processes"@en-AU ;
    skos:narrower C1901A00006:806 ;
    skos:prefLabel "Item I810"@en-AU ;
    dcat:accessURL "https://www.legislation.gov.au/C1901A00006/2024-07-01/2024-07-01/text/original/epub/OEBPS/document_2/document_2.html#_Toc172624565"^^xsd:anyURI .

C1901A00006:812 a legcons:Item,
        skos:Concept,
        dcat:Resource ;
    rdfs:label "Item I812"@en-AU ;
    rdfs:comment "153 ZQI  Consignment - GraphNodeID: I812"@en-AU ;
    skos:definition "153 ZQI  Consignment"@en-AU ;
    skos:narrower C1901A00006:811 ;
    skos:prefLabel "Item I812"@en-AU ;
    dcat:accessURL "https://www.legislation.gov.au/C1901A00006/2024-07-01/2024-07-01/text/original/epub/OEBPS/document_2/document_2.html#_Toc172624567"^^xsd:anyURI .

C1901A00006:814 a legcons:Item,
        skos:Concept,
        dcat:Resource ;
    rdfs:label "Item I814"@en-AU ;
    rdfs:comment "153 ZQJ  Regulations - GraphNodeID: I814"@en-AU ;
    skos:definition "153 ZQJ  Regulations"@en-AU ;
    skos:narrower C1901A00006:813 ;
    skos:prefLabel "Item I814"@en-AU ;
    dcat:accessURL "https://www.legislation.gov.au/C1901A00006/2024-07-01/2024-07-01/text/original/epub/OEBPS/document_2/document_2.html#_Toc172624569"^^xsd:anyURI .

C1901A00006:817 a legcons:Item,
        skos:Concept,
        dcat:Resource ;
    rdfs:label "Item I817"@en-AU ;
    rdfs:comment "153 ZRA  Simplified outline of this Division - GraphNodeID: I817"@en-AU ;
    skos:definition "153 ZRA  Simplified outline of this Division"@en-AU ;
    skos:narrower C1901A00006:816 ;
    skos:prefLabel "Item I817"@en-AU ;
    dcat:accessURL "https://www.legislation.gov.au/C1901A00006/2024-07-01/2024-07-01/text/original/epub/OEBPS/document_2/document_2.html#_Toc172624572"^^xsd:anyURI .

C1901A00006:818 a legcons:Item,
        skos:Concept,
        dcat:Resource ;
    rdfs:label "Item I818"@en-AU ;
    rdfs:comment "153 ZRB  Interpretation - GraphNodeID: I818"@en-AU ;
    skos:definition "153 ZRB  Interpretation"@en-AU ;
    skos:narrower C1901A00006:816 ;
    skos:prefLabel "Item I818"@en-AU ;
    dcat:accessURL "https://www.legislation.gov.au/C1901A00006/2024-07-01/2024-07-01/text/original/epub/OEBPS/document_2/document_2.html#_Toc172624573"^^xsd:anyURI .

C1901A00006:82 a legcons:Item,
        skos:Concept,
        dcat:Resource ;
    rdfs:label "Item I82"@en-AU ;
    rdfs:comment "64 AB  Cargo reports - GraphNodeID: I82"@en-AU ;
    skos:definition "64 AB  Cargo reports"@en-AU ;
    skos:narrower C1901A00006:75 ;
    skos:prefLabel "Item I82"@en-AU ;
    dcat:accessURL "https://www.legislation.gov.au/C1901A00006/2024-07-01/2024-07-01/text/original/epub/OEBPS/document_1/document_1.html#_Toc172623056"^^xsd:anyURI .

C1901A00006:820 a legcons:Item,
        skos:Concept,
        dcat:Resource ;
    rdfs:label "Item I820"@en-AU ;
    rdfs:comment "153 ZRC  Goods wholly obtained or produced in the United Kingdom or in the United Kingdom and Australia - GraphNodeID: I820"@en-AU ;
    skos:definition "153 ZRC  Goods wholly obtained or produced in the United Kingdom or in the United Kingdom and Australia"@en-AU ;
    skos:narrower C1901A00006:819 ;
    skos:prefLabel "Item I820"@en-AU ;
    dcat:accessURL "https://www.legislation.gov.au/C1901A00006/2024-07-01/2024-07-01/text/original/epub/OEBPS/document_2/document_2.html#_Toc172624575"^^xsd:anyURI .

C1901A00006:822 a legcons:Item,
        skos:Concept,
        dcat:Resource ;
    rdfs:label "Item I822"@en-AU ;
    rdfs:comment "153 ZRD  Goods produced in the United Kingdom or in the United Kingdom and Australia from originating materials - GraphNodeID: I822"@en-AU ;
    skos:definition "153 ZRD  Goods produced in the United Kingdom or in the United Kingdom and Australia from originating materials"@en-AU ;
    skos:narrower C1901A00006:821 ;
    skos:prefLabel "Item I822"@en-AU ;
    dcat:accessURL "https://www.legislation.gov.au/C1901A00006/2024-07-01/2024-07-01/text/original/epub/OEBPS/document_2/document_2.html#_Toc172624577"^^xsd:anyURI .

C1901A00006:824 a legcons:Item,
        skos:Concept,
        dcat:Resource ;
    rdfs:label "Item I824"@en-AU ;
    rdfs:comment "153 ZRE  Goods produced in the United Kingdom or in the United Kingdom and Australia from non originating materials - GraphNodeID: I824"@en-AU ;
    skos:definition "153 ZRE  Goods produced in the United Kingdom or in the United Kingdom and Australia from non originating materials"@en-AU ;
    skos:narrower C1901A00006:823 ;
    skos:prefLabel "Item I824"@en-AU ;
    dcat:accessURL "https://www.legislation.gov.au/C1901A00006/2024-07-01/2024-07-01/text/original/epub/OEBPS/document_2/document_2.html#_Toc172624579"^^xsd:anyURI .

C1901A00006:825 a legcons:Item,
        skos:Concept,
        dcat:Resource ;
    rdfs:label "Item I825"@en-AU ;
    rdfs:comment "153 ZRF  Packaging materials and containers - GraphNodeID: I825"@en-AU ;
    skos:definition "153 ZRF  Packaging materials and containers"@en-AU ;
    skos:narrower C1901A00006:823 ;
    skos:prefLabel "Item I825"@en-AU ;
    dcat:accessURL "https://www.legislation.gov.au/C1901A00006/2024-07-01/2024-07-01/text/original/epub/OEBPS/document_2/document_2.html#_Toc172624580"^^xsd:anyURI .

C1901A00006:827 a legcons:Item,
        skos:Concept,
        dcat:Resource ;
    rdfs:label "Item I827"@en-AU ;
    rdfs:comment "153 ZRG  Goods that are accessories spare parts tools or instructional or other information materials - GraphNodeID: I827"@en-AU ;
    skos:definition "153 ZRG  Goods that are accessories spare parts tools or instructional or other information materials"@en-AU ;
    skos:narrower C1901A00006:826 ;
    skos:prefLabel "Item I827"@en-AU ;
    dcat:accessURL "https://www.legislation.gov.au/C1901A00006/2024-07-01/2024-07-01/text/original/epub/OEBPS/document_2/document_2.html#_Toc172624582"^^xsd:anyURI .

C1901A00006:829 a legcons:Item,
        skos:Concept,
        dcat:Resource ;
    rdfs:label "Item I829"@en-AU ;
    rdfs:comment "153 ZRH  Consignment - GraphNodeID: I829"@en-AU ;
    skos:definition "153 ZRH  Consignment"@en-AU ;
    skos:narrower C1901A00006:828 ;
    skos:prefLabel "Item I829"@en-AU ;
    dcat:accessURL "https://www.legislation.gov.au/C1901A00006/2024-07-01/2024-07-01/text/original/epub/OEBPS/document_2/document_2.html#_Toc172624584"^^xsd:anyURI .

C1901A00006:83 a legcons:Item,
        skos:Concept,
        dcat:Resource ;
    rdfs:label "Item I83"@en-AU ;
    rdfs:comment "64 ABAA  Outturn reports - GraphNodeID: I83"@en-AU ;
    skos:definition "64 ABAA  Outturn reports"@en-AU ;
    skos:narrower C1901A00006:75 ;
    skos:prefLabel "Item I83"@en-AU ;
    dcat:accessURL "https://www.legislation.gov.au/C1901A00006/2024-07-01/2024-07-01/text/original/epub/OEBPS/document_1/document_1.html#_Toc172623057"^^xsd:anyURI .

C1901A00006:831 a legcons:Item,
        skos:Concept,
        dcat:Resource ;
    rdfs:label "Item I831"@en-AU ;
    rdfs:comment "153 ZRI  Regulations - GraphNodeID: I831"@en-AU ;
    skos:definition "153 ZRI  Regulations"@en-AU ;
    skos:narrower C1901A00006:830 ;
    skos:prefLabel "Item I831"@en-AU ;
    dcat:accessURL "https://www.legislation.gov.au/C1901A00006/2024-07-01/2024-07-01/text/original/epub/OEBPS/document_2/document_2.html#_Toc172624586"^^xsd:anyURI .

C1901A00006:832 a legcons:Division,
        skos:Concept,
        dcat:Resource ;
    rdfs:label "Division D832"@en-AU ;
    rdfs:comment "Division 2 Valuation of imported goods - GraphNodeID: D832"@en-AU ;
    skos:definition "Division 2 Valuation of imported goods"@en-AU ;
    skos:narrower C1901A00006:475 ;
    skos:prefLabel "Division D832"@en-AU ;
    dcat:accessURL "https://www.legislation.gov.au/C1901A00006/2024-07-01/2024-07-01/text/original/epub/OEBPS/document_2/document_2.html#_Toc172624587"^^xsd:anyURI .

C1901A00006:833 a legcons:Item,
        skos:Concept,
        dcat:Resource ;
    rdfs:label "Item I833"@en-AU ;
    rdfs:comment "154  Interpretation - GraphNodeID: I833"@en-AU ;
    skos:definition "154  Interpretation"@en-AU ;
    skos:narrower C1901A00006:830 ;
    skos:prefLabel "Item I833"@en-AU ;
    dcat:accessURL "https://www.legislation.gov.au/C1901A00006/2024-07-01/2024-07-01/text/original/epub/OEBPS/document_2/document_2.html#_Toc172624588"^^xsd:anyURI .

C1901A00006:834 a legcons:Item,
        skos:Concept,
        dcat:Resource ;
    rdfs:label "Item I834"@en-AU ;
    rdfs:comment "155  InterpretationBuying commission - GraphNodeID: I834"@en-AU ;
    skos:definition "155  InterpretationBuying commission"@en-AU ;
    skos:narrower C1901A00006:830 ;
    skos:prefLabel "Item I834"@en-AU ;
    dcat:accessURL "https://www.legislation.gov.au/C1901A00006/2024-07-01/2024-07-01/text/original/epub/OEBPS/document_2/document_2.html#_Toc172624589"^^xsd:anyURI .

C1901A00006:835 a legcons:Item,
        skos:Concept,
        dcat:Resource ;
    rdfs:label "Item I835"@en-AU ;
    rdfs:comment "156  InterpretationIdentical goods and similar goods - GraphNodeID: I835"@en-AU ;
    skos:definition "156  InterpretationIdentical goods and similar goods"@en-AU ;
    skos:narrower C1901A00006:830 ;
    skos:prefLabel "Item I835"@en-AU ;
    dcat:accessURL "https://www.legislation.gov.au/C1901A00006/2024-07-01/2024-07-01/text/original/epub/OEBPS/document_2/document_2.html#_Toc172624590"^^xsd:anyURI .

C1901A00006:836 a legcons:Item,
        skos:Concept,
        dcat:Resource ;
    rdfs:label "Item I836"@en-AU ;
    rdfs:comment "157  InterpretationRoyalties - GraphNodeID: I836"@en-AU ;
    skos:definition "157  InterpretationRoyalties"@en-AU ;
    skos:narrower C1901A00006:830 ;
    skos:prefLabel "Item I836"@en-AU ;
    dcat:accessURL "https://www.legislation.gov.au/C1901A00006/2024-07-01/2024-07-01/text/original/epub/OEBPS/document_2/document_2.html#_Toc172624591"^^xsd:anyURI .

C1901A00006:837 a legcons:Item,
        skos:Concept,
        dcat:Resource ;
    rdfs:label "Item I837"@en-AU ;
    rdfs:comment "158  InterpretationTransportation costs - GraphNodeID: I837"@en-AU ;
    skos:definition "158  InterpretationTransportation costs"@en-AU ;
    skos:narrower C1901A00006:830 ;
    skos:prefLabel "Item I837"@en-AU ;
    dcat:accessURL "https://www.legislation.gov.au/C1901A00006/2024-07-01/2024-07-01/text/original/epub/OEBPS/document_2/document_2.html#_Toc172624592"^^xsd:anyURI .

C1901A00006:838 a legcons:Item,
        skos:Concept,
        dcat:Resource ;
    rdfs:label "Item I838"@en-AU ;
    rdfs:comment "159  Value of imported goods - GraphNodeID: I838"@en-AU ;
    skos:definition "159  Value of imported goods"@en-AU ;
    skos:narrower C1901A00006:830 ;
    skos:prefLabel "Item I838"@en-AU ;
    dcat:accessURL "https://www.legislation.gov.au/C1901A00006/2024-07-01/2024-07-01/text/original/epub/OEBPS/document_2/document_2.html#_Toc172624593"^^xsd:anyURI .

C1901A00006:839 a legcons:Item,
        skos:Concept,
        dcat:Resource ;
    rdfs:label "Item I839"@en-AU ;
    rdfs:comment "160  Inability to determine a value of imported goods by reason of insufficient or unreliable information - GraphNodeID: I839"@en-AU ;
    skos:definition "160  Inability to determine a value of imported goods by reason of insufficient or unreliable information"@en-AU ;
    skos:narrower C1901A00006:830 ;
    skos:prefLabel "Item I839"@en-AU ;
    dcat:accessURL "https://www.legislation.gov.au/C1901A00006/2024-07-01/2024-07-01/text/original/epub/OEBPS/document_2/document_2.html#_Toc172624594"^^xsd:anyURI .

C1901A00006:84 a legcons:Item,
        skos:Concept,
        dcat:Resource ;
    rdfs:label "Item I84"@en-AU ;
    rdfs:comment "64 ABAB  When outturn report is to be communicated to Department - GraphNodeID: I84"@en-AU ;
    skos:definition "64 ABAB  When outturn report is to be communicated to Department"@en-AU ;
    skos:narrower C1901A00006:75 ;
    skos:prefLabel "Item I84"@en-AU ;
    dcat:accessURL "https://www.legislation.gov.au/C1901A00006/2024-07-01/2024-07-01/text/original/epub/OEBPS/document_1/document_1.html#_Toc172623058"^^xsd:anyURI .

C1901A00006:840 a legcons:Item,
        skos:Concept,
        dcat:Resource ;
    rdfs:label "Item I840"@en-AU ;
    rdfs:comment "161  Transaction value - GraphNodeID: I840"@en-AU ;
    skos:definition "161  Transaction value"@en-AU ;
    skos:narrower C1901A00006:830 ;
    skos:prefLabel "Item I840"@en-AU ;
    dcat:accessURL "https://www.legislation.gov.au/C1901A00006/2024-07-01/2024-07-01/text/original/epub/OEBPS/document_2/document_2.html#_Toc172624595"^^xsd:anyURI .

C1901A00006:841 a legcons:Item,
        skos:Concept,
        dcat:Resource ;
    rdfs:label "Item I841"@en-AU ;
    rdfs:comment "161 A  Identical goods value - GraphNodeID: I841"@en-AU ;
    skos:definition "161 A  Identical goods value"@en-AU ;
    skos:narrower C1901A00006:830 ;
    skos:prefLabel "Item I841"@en-AU ;
    dcat:accessURL "https://www.legislation.gov.au/C1901A00006/2024-07-01/2024-07-01/text/original/epub/OEBPS/document_2/document_2.html#_Toc172624596"^^xsd:anyURI .

C1901A00006:842 a legcons:Item,
        skos:Concept,
        dcat:Resource ;
    rdfs:label "Item I842"@en-AU ;
    rdfs:comment "161 B  Similar goods value - GraphNodeID: I842"@en-AU ;
    skos:definition "161 B  Similar goods value"@en-AU ;
    skos:narrower C1901A00006:830 ;
    skos:prefLabel "Item I842"@en-AU ;
    dcat:accessURL "https://www.legislation.gov.au/C1901A00006/2024-07-01/2024-07-01/text/original/epub/OEBPS/document_2/document_2.html#_Toc172624597"^^xsd:anyURI .

C1901A00006:843 a legcons:Item,
        skos:Concept,
        dcat:Resource ;
    rdfs:label "Item I843"@en-AU ;
    rdfs:comment "161 C  Deductive contemporary sales value - GraphNodeID: I843"@en-AU ;
    skos:definition "161 C  Deductive contemporary sales value"@en-AU ;
    skos:narrower C1901A00006:830 ;
    skos:prefLabel "Item I843"@en-AU ;
    dcat:accessURL "https://www.legislation.gov.au/C1901A00006/2024-07-01/2024-07-01/text/original/epub/OEBPS/document_2/document_2.html#_Toc172624598"^^xsd:anyURI .

C1901A00006:844 a legcons:Item,
        skos:Concept,
        dcat:Resource ;
    rdfs:label "Item I844"@en-AU ;
    rdfs:comment "161 D  Deductive later sales value - GraphNodeID: I844"@en-AU ;
    skos:definition "161 D  Deductive later sales value"@en-AU ;
    skos:narrower C1901A00006:830 ;
    skos:prefLabel "Item I844"@en-AU ;
    dcat:accessURL "https://www.legislation.gov.au/C1901A00006/2024-07-01/2024-07-01/text/original/epub/OEBPS/document_2/document_2.html#_Toc172624599"^^xsd:anyURI .

C1901A00006:845 a legcons:Item,
        skos:Concept,
        dcat:Resource ;
    rdfs:label "Item I845"@en-AU ;
    rdfs:comment "161 E  Deductive derived goods sales value - GraphNodeID: I845"@en-AU ;
    skos:definition "161 E  Deductive derived goods sales value"@en-AU ;
    skos:narrower C1901A00006:830 ;
    skos:prefLabel "Item I845"@en-AU ;
    dcat:accessURL "https://www.legislation.gov.au/C1901A00006/2024-07-01/2024-07-01/text/original/epub/OEBPS/document_2/document_2.html#_Toc172624600"^^xsd:anyURI .

C1901A00006:846 a legcons:Item,
        skos:Concept,
        dcat:Resource ;
    rdfs:label "Item I846"@en-AU ;
    rdfs:comment "161 F  Computed value - GraphNodeID: I846"@en-AU ;
    skos:definition "161 F  Computed value"@en-AU ;
    skos:narrower C1901A00006:830 ;
    skos:prefLabel "Item I846"@en-AU ;
    dcat:accessURL "https://www.legislation.gov.au/C1901A00006/2024-07-01/2024-07-01/text/original/epub/OEBPS/document_2/document_2.html#_Toc172624601"^^xsd:anyURI .

C1901A00006:847 a legcons:Item,
        skos:Concept,
        dcat:Resource ;
    rdfs:label "Item I847"@en-AU ;
    rdfs:comment "161 G  Fall back value - GraphNodeID: I847"@en-AU ;
    skos:definition "161 G  Fall back value"@en-AU ;
    skos:narrower C1901A00006:830 ;
    skos:prefLabel "Item I847"@en-AU ;
    dcat:accessURL "https://www.legislation.gov.au/C1901A00006/2024-07-01/2024-07-01/text/original/epub/OEBPS/document_2/document_2.html#_Toc172624602"^^xsd:anyURI .

C1901A00006:848 a legcons:Item,
        skos:Concept,
        dcat:Resource ;
    rdfs:label "Item I848"@en-AU ;
    rdfs:comment "161 H  When transaction value unable to be determined - GraphNodeID: I848"@en-AU ;
    skos:definition "161 H  When transaction value unable to be determined"@en-AU ;
    skos:narrower C1901A00006:830 ;
    skos:prefLabel "Item I848"@en-AU ;
    dcat:accessURL "https://www.legislation.gov.au/C1901A00006/2024-07-01/2024-07-01/text/original/epub/OEBPS/document_2/document_2.html#_Toc172624603"^^xsd:anyURI .

C1901A00006:849 a legcons:Item,
        skos:Concept,
        dcat:Resource ;
    rdfs:label "Item I849"@en-AU ;
    rdfs:comment "161 J  Value of goods to be in Australian currency - GraphNodeID: I849"@en-AU ;
    skos:definition "161 J  Value of goods to be in Australian currency"@en-AU ;
    skos:narrower C1901A00006:830 ;
    skos:prefLabel "Item I849"@en-AU ;
    dcat:accessURL "https://www.legislation.gov.au/C1901A00006/2024-07-01/2024-07-01/text/original/epub/OEBPS/document_2/document_2.html#_Toc172624604"^^xsd:anyURI .

C1901A00006:85 a legcons:Item,
        skos:Concept,
        dcat:Resource ;
    rdfs:label "Item I85"@en-AU ;
    rdfs:comment "64 ABAC  Explanation of shortlanded or surplus cargo - GraphNodeID: I85"@en-AU ;
    skos:definition "64 ABAC  Explanation of shortlanded or surplus cargo"@en-AU ;
    skos:narrower C1901A00006:75 ;
    skos:prefLabel "Item I85"@en-AU ;
    dcat:accessURL "https://www.legislation.gov.au/C1901A00006/2024-07-01/2024-07-01/text/original/epub/OEBPS/document_1/document_1.html#_Toc172623059"^^xsd:anyURI .

C1901A00006:850 a legcons:Item,
        skos:Concept,
        dcat:Resource ;
    rdfs:label "Item I850"@en-AU ;
    rdfs:comment "161 K  Owner to be advised of value of goods - GraphNodeID: I850"@en-AU ;
    skos:definition "161 K  Owner to be advised of value of goods"@en-AU ;
    skos:narrower C1901A00006:830 ;
    skos:prefLabel "Item I850"@en-AU ;
    dcat:accessURL "https://www.legislation.gov.au/C1901A00006/2024-07-01/2024-07-01/text/original/epub/OEBPS/document_2/document_2.html#_Toc172624605"^^xsd:anyURI .

C1901A00006:851 a legcons:Item,
        skos:Concept,
        dcat:Resource ;
    rdfs:label "Item I851"@en-AU ;
    rdfs:comment "161 L  Review of determinations and other decisions - GraphNodeID: I851"@en-AU ;
    skos:definition "161 L  Review of determinations and other decisions"@en-AU ;
    skos:narrower C1901A00006:830 ;
    skos:prefLabel "Item I851"@en-AU ;
    dcat:accessURL "https://www.legislation.gov.au/C1901A00006/2024-07-01/2024-07-01/text/original/epub/OEBPS/document_2/document_2.html#_Toc172624606"^^xsd:anyURI .

C1901A00006:852 a legcons:Division,
        skos:Concept,
        dcat:Resource ;
    rdfs:label "Division D852"@en-AU ;
    rdfs:comment "Division 3 Payment and recovery of deposits refunds unpaid duty etc - GraphNodeID: D852"@en-AU ;
    skos:definition "Division 3 Payment and recovery of deposits refunds unpaid duty etc"@en-AU ;
    skos:narrower C1901A00006:475 ;
    skos:prefLabel "Division D852"@en-AU ;
    dcat:accessURL "https://www.legislation.gov.au/C1901A00006/2024-07-01/2024-07-01/text/original/epub/OEBPS/document_2/document_2.html#_Toc172624607"^^xsd:anyURI .

C1901A00006:853 a legcons:Item,
        skos:Concept,
        dcat:Resource ;
    rdfs:label "Item I853"@en-AU ;
    rdfs:comment "162  Delivery of goods upon giving of security or undertaking for payment of duty GST and luxury car tax - GraphNodeID: I853"@en-AU ;
    skos:definition "162  Delivery of goods upon giving of security or undertaking for payment of duty GST and luxury car tax"@en-AU ;
    skos:narrower C1901A00006:830 ;
    skos:prefLabel "Item I853"@en-AU ;
    dcat:accessURL "https://www.legislation.gov.au/C1901A00006/2024-07-01/2024-07-01/text/original/epub/OEBPS/document_2/document_2.html#_Toc172624608"^^xsd:anyURI .

C1901A00006:854 a legcons:Item,
        skos:Concept,
        dcat:Resource ;
    rdfs:label "Item I854"@en-AU ;
    rdfs:comment "162 A  Delivery of goods on the giving of a general security or undertaking for payment of duty GST and luxury car tax - GraphNodeID: I854"@en-AU ;
    skos:definition "162 A  Delivery of goods on the giving of a general security or undertaking for payment of duty GST and luxury car tax"@en-AU ;
    skos:narrower C1901A00006:830 ;
    skos:prefLabel "Item I854"@en-AU ;
    dcat:accessURL "https://www.legislation.gov.au/C1901A00006/2024-07-01/2024-07-01/text/original/epub/OEBPS/document_2/document_2.html#_Toc172624609"^^xsd:anyURI .

C1901A00006:855 a legcons:Item,
        skos:Concept,
        dcat:Resource ;
    rdfs:label "Item I855"@en-AU ;
    rdfs:comment "162 AA  Applications to deal with goods imported temporarily without duty - GraphNodeID: I855"@en-AU ;
    skos:definition "162 AA  Applications to deal with goods imported temporarily without duty"@en-AU ;
    skos:narrower C1901A00006:830 ;
    skos:prefLabel "Item I855"@en-AU ;
    dcat:accessURL "https://www.legislation.gov.au/C1901A00006/2024-07-01/2024-07-01/text/original/epub/OEBPS/document_2/document_2.html#_Toc172624610"^^xsd:anyURI .

C1901A00006:856 a legcons:Item,
        skos:Concept,
        dcat:Resource ;
    rdfs:label "Item I856"@en-AU ;
    rdfs:comment "162 B  Pallets used in international transport - GraphNodeID: I856"@en-AU ;
    skos:definition "162 B  Pallets used in international transport"@en-AU ;
    skos:narrower C1901A00006:830 ;
    skos:prefLabel "Item I856"@en-AU ;
    dcat:accessURL "https://www.legislation.gov.au/C1901A00006/2024-07-01/2024-07-01/text/original/epub/OEBPS/document_2/document_2.html#_Toc172624611"^^xsd:anyURI .

C1901A00006:857 a legcons:Item,
        skos:Concept,
        dcat:Resource ;
    rdfs:label "Item I857"@en-AU ;
    rdfs:comment "163  Refunds etc of duty - GraphNodeID: I857"@en-AU ;
    skos:definition "163  Refunds etc of duty"@en-AU ;
    skos:narrower C1901A00006:830 ;
    skos:prefLabel "Item I857"@en-AU ;
    dcat:accessURL "https://www.legislation.gov.au/C1901A00006/2024-07-01/2024-07-01/text/original/epub/OEBPS/document_2/document_2.html#_Toc172624612"^^xsd:anyURI .

C1901A00006:858 a legcons:Item,
        skos:Concept,
        dcat:Resource ;
    rdfs:label "Item I858"@en-AU ;
    rdfs:comment "164 B  Refunds of export duty - GraphNodeID: I858"@en-AU ;
    skos:definition "164 B  Refunds of export duty"@en-AU ;
    skos:narrower C1901A00006:830 ;
    skos:prefLabel "Item I858"@en-AU ;
    dcat:accessURL "https://www.legislation.gov.au/C1901A00006/2024-07-01/2024-07-01/text/original/epub/OEBPS/document_2/document_2.html#_Toc172624613"^^xsd:anyURI .

C1901A00006:859 a legcons:Item,
        skos:Concept,
        dcat:Resource ;
    rdfs:label "Item I859"@en-AU ;
    rdfs:comment "165  Recovery of unpaid duty etc - GraphNodeID: I859"@en-AU ;
    skos:definition "165  Recovery of unpaid duty etc"@en-AU ;
    skos:narrower C1901A00006:830 ;
    skos:prefLabel "Item I859"@en-AU ;
    dcat:accessURL "https://www.legislation.gov.au/C1901A00006/2024-07-01/2024-07-01/text/original/epub/OEBPS/document_2/document_2.html#_Toc172624614"^^xsd:anyURI .

C1901A00006:86 a legcons:Item,
        skos:Concept,
        dcat:Resource ;
    rdfs:label "Item I86"@en-AU ;
    rdfs:comment "64 ACA  Passenger reports - GraphNodeID: I86"@en-AU ;
    skos:definition "64 ACA  Passenger reports"@en-AU ;
    skos:narrower C1901A00006:75 ;
    skos:prefLabel "Item I86"@en-AU ;
    dcat:accessURL "https://www.legislation.gov.au/C1901A00006/2024-07-01/2024-07-01/text/original/epub/OEBPS/document_1/document_1.html#_Toc172623060"^^xsd:anyURI .

C1901A00006:860 a legcons:Item,
        skos:Concept,
        dcat:Resource ;
    rdfs:label "Item I860"@en-AU ;
    rdfs:comment "165 A  Refunds etc may be applied against unpaid duty - GraphNodeID: I860"@en-AU ;
    skos:definition "165 A  Refunds etc may be applied against unpaid duty"@en-AU ;
    skos:narrower C1901A00006:830 ;
    skos:prefLabel "Item I860"@en-AU ;
    dcat:accessURL "https://www.legislation.gov.au/C1901A00006/2024-07-01/2024-07-01/text/original/epub/OEBPS/document_2/document_2.html#_Toc172624615"^^xsd:anyURI .

C1901A00006:861 a legcons:Item,
        skos:Concept,
        dcat:Resource ;
    rdfs:label "Item I861"@en-AU ;
    rdfs:comment "166  No refund if duty altered - GraphNodeID: I861"@en-AU ;
    skos:definition "166  No refund if duty altered"@en-AU ;
    skos:narrower C1901A00006:830 ;
    skos:prefLabel "Item I861"@en-AU ;
    dcat:accessURL "https://www.legislation.gov.au/C1901A00006/2024-07-01/2024-07-01/text/original/epub/OEBPS/document_2/document_2.html#_Toc172624616"^^xsd:anyURI .

C1901A00006:862 a legcons:Division,
        skos:Concept,
        dcat:Resource ;
    rdfs:label "Division D862"@en-AU ;
    rdfs:comment "Division 4 Disputes as to duty - GraphNodeID: D862"@en-AU ;
    skos:definition "Division 4 Disputes as to duty"@en-AU ;
    skos:narrower C1901A00006:475 ;
    skos:prefLabel "Division D862"@en-AU ;
    dcat:accessURL "https://www.legislation.gov.au/C1901A00006/2024-07-01/2024-07-01/text/original/epub/OEBPS/document_2/document_2.html#_Toc172624617"^^xsd:anyURI .

C1901A00006:863 a legcons:Item,
        skos:Concept,
        dcat:Resource ;
    rdfs:label "Item I863"@en-AU ;
    rdfs:comment "167  Payments under protest - GraphNodeID: I863"@en-AU ;
    skos:definition "167  Payments under protest"@en-AU ;
    skos:narrower C1901A00006:830 ;
    skos:prefLabel "Item I863"@en-AU ;
    dcat:accessURL "https://www.legislation.gov.au/C1901A00006/2024-07-01/2024-07-01/text/original/epub/OEBPS/document_2/document_2.html#_Toc172624618"^^xsd:anyURI .

C1901A00006:864 a legcons:Part,
        skos:Concept,
        dcat:Resource ;
    rdfs:label "Part P864"@en-AU ;
    rdfs:comment "Part IXDrawbacks - GraphNodeID: P864"@en-AU ;
    skos:definition "Part IXDrawbacks"@en-AU ;
    skos:narrower C1901A00006:456 ;
    skos:prefLabel "Part P864"@en-AU ;
    dcat:accessURL "https://www.legislation.gov.au/C1901A00006/2024-07-01/2024-07-01/text/original/epub/OEBPS/document_2/document_2.html#_Toc172624619"^^xsd:anyURI .

C1901A00006:865 a legcons:Item,
        skos:Concept,
        dcat:Resource ;
    rdfs:label "Item I865"@en-AU ;
    rdfs:comment "168  Drawbacks of import duty - GraphNodeID: I865"@en-AU ;
    skos:definition "168  Drawbacks of import duty"@en-AU ;
    skos:narrower C1901A00006:830 ;
    skos:prefLabel "Item I865"@en-AU ;
    dcat:accessURL "https://www.legislation.gov.au/C1901A00006/2024-07-01/2024-07-01/text/original/epub/OEBPS/document_2/document_2.html#_Toc172624620"^^xsd:anyURI .

C1901A00006:866 a legcons:Part,
        skos:Concept,
        dcat:Resource ;
    rdfs:label "Part P866"@en-AU ;
    rdfs:comment "Part XThe coasting trade - GraphNodeID: P866"@en-AU ;
    skos:definition "Part XThe coasting trade"@en-AU ;
    skos:narrower C1901A00006:456 ;
    skos:prefLabel "Part P866"@en-AU ;
    dcat:accessURL "https://www.legislation.gov.au/C1901A00006/2024-07-01/2024-07-01/text/original/epub/OEBPS/document_2/document_2.html#_Toc172624621"^^xsd:anyURI .

C1901A00006:867 a legcons:Item,
        skos:Concept,
        dcat:Resource ;
    rdfs:label "Item I867"@en-AU ;
    rdfs:comment "175  Goods not to be transferred between certain vessels - GraphNodeID: I867"@en-AU ;
    skos:definition "175  Goods not to be transferred between certain vessels"@en-AU ;
    skos:narrower C1901A00006:830 ;
    skos:prefLabel "Item I867"@en-AU ;
    dcat:accessURL "https://www.legislation.gov.au/C1901A00006/2024-07-01/2024-07-01/text/original/epub/OEBPS/document_2/document_2.html#_Toc172624622"^^xsd:anyURI .

C1901A00006:869 a legcons:Division,
        skos:Concept,
        dcat:Resource ;
    rdfs:label "Division D869"@en-AU ;
    rdfs:comment "Division 1 Preliminary - GraphNodeID: D869"@en-AU ;
    skos:definition "Division 1 Preliminary"@en-AU ;
    skos:narrower C1901A00006:868 ;
    skos:prefLabel "Division D869"@en-AU ;
    dcat:accessURL "https://www.legislation.gov.au/C1901A00006/2024-07-01/2024-07-01/text/original/epub/OEBPS/document_2/document_2.html#_Toc172624624"^^xsd:anyURI .

C1901A00006:87 a legcons:Item,
        skos:Concept,
        dcat:Resource ;
    rdfs:label "Item I87"@en-AU ;
    rdfs:comment "64 ACB  Crew reports - GraphNodeID: I87"@en-AU ;
    skos:definition "64 ACB  Crew reports"@en-AU ;
    skos:narrower C1901A00006:75 ;
    skos:prefLabel "Item I87"@en-AU ;
    dcat:accessURL "https://www.legislation.gov.au/C1901A00006/2024-07-01/2024-07-01/text/original/epub/OEBPS/document_1/document_1.html#_Toc172623061"^^xsd:anyURI .

C1901A00006:870 a legcons:Item,
        skos:Concept,
        dcat:Resource ;
    rdfs:label "Item I870"@en-AU ;
    rdfs:comment "176  Establishment of the Australian Trusted Trader Programme - GraphNodeID: I870"@en-AU ;
    skos:definition "176  Establishment of the Australian Trusted Trader Programme"@en-AU ;
    skos:narrower C1901A00006:830 ;
    skos:prefLabel "Item I870"@en-AU ;
    dcat:accessURL "https://www.legislation.gov.au/C1901A00006/2024-07-01/2024-07-01/text/original/epub/OEBPS/document_2/document_2.html#_Toc172624625"^^xsd:anyURI .

C1901A00006:873 a legcons:Item,
        skos:Concept,
        dcat:Resource ;
    rdfs:label "Item I873"@en-AU ;
    rdfs:comment "176 A  Trusted trader agreement may be entered into - GraphNodeID: I873"@en-AU ;
    skos:definition "176 A  Trusted trader agreement may be entered into"@en-AU ;
    skos:narrower C1901A00006:872 ;
    skos:prefLabel "Item I873"@en-AU ;
    dcat:accessURL "https://www.legislation.gov.au/C1901A00006/2024-07-01/2024-07-01/text/original/epub/OEBPS/document_2/document_2.html#_Toc172624628"^^xsd:anyURI .

C1901A00006:874 a legcons:Item,
        skos:Concept,
        dcat:Resource ;
    rdfs:label "Item I874"@en-AU ;
    rdfs:comment "176 B  Nomination process - GraphNodeID: I874"@en-AU ;
    skos:definition "176 B  Nomination process"@en-AU ;
    skos:narrower C1901A00006:872 ;
    skos:prefLabel "Item I874"@en-AU ;
    dcat:accessURL "https://www.legislation.gov.au/C1901A00006/2024-07-01/2024-07-01/text/original/epub/OEBPS/document_2/document_2.html#_Toc172624629"^^xsd:anyURI .

C1901A00006:876 a legcons:Item,
        skos:Concept,
        dcat:Resource ;
    rdfs:label "Item I876"@en-AU ;
    rdfs:comment "178  Terms and conditions of trusted trader agreements - GraphNodeID: I876"@en-AU ;
    skos:definition "178  Terms and conditions of trusted trader agreements"@en-AU ;
    skos:narrower C1901A00006:875 ;
    skos:prefLabel "Item I876"@en-AU ;
    dcat:accessURL "https://www.legislation.gov.au/C1901A00006/2024-07-01/2024-07-01/text/original/epub/OEBPS/document_2/document_2.html#_Toc172624631"^^xsd:anyURI .

C1901A00006:877 a legcons:Item,
        skos:Concept,
        dcat:Resource ;
    rdfs:label "Item I877"@en-AU ;
    rdfs:comment "178 A  Variation suspension or termination of trusted trader agreements - GraphNodeID: I877"@en-AU ;
    skos:definition "178 A  Variation suspension or termination of trusted trader agreements"@en-AU ;
    skos:narrower C1901A00006:875 ;
    skos:prefLabel "Item I877"@en-AU ;
    dcat:accessURL "https://www.legislation.gov.au/C1901A00006/2024-07-01/2024-07-01/text/original/epub/OEBPS/document_2/document_2.html#_Toc172624632"^^xsd:anyURI .

C1901A00006:878 a legcons:Division,
        skos:Concept,
        dcat:Resource ;
    rdfs:label "Division D878"@en-AU ;
    rdfs:comment "Division 3 Register of Trusted Trader Agreements - GraphNodeID: D878"@en-AU ;
    skos:definition "Division 3 Register of Trusted Trader Agreements"@en-AU ;
    skos:narrower C1901A00006:868 ;
    skos:prefLabel "Division D878"@en-AU ;
    dcat:accessURL "https://www.legislation.gov.au/C1901A00006/2024-07-01/2024-07-01/text/original/epub/OEBPS/document_2/document_2.html#_Toc172624633"^^xsd:anyURI .

C1901A00006:879 a legcons:Item,
        skos:Concept,
        dcat:Resource ;
    rdfs:label "Item I879"@en-AU ;
    rdfs:comment "178 B  Register of Trusted Trader Agreements - GraphNodeID: I879"@en-AU ;
    skos:definition "178 B  Register of Trusted Trader Agreements"@en-AU ;
    skos:narrower C1901A00006:875 ;
    skos:prefLabel "Item I879"@en-AU ;
    dcat:accessURL "https://www.legislation.gov.au/C1901A00006/2024-07-01/2024-07-01/text/original/epub/OEBPS/document_2/document_2.html#_Toc172624634"^^xsd:anyURI .

C1901A00006:88 a legcons:Item,
        skos:Concept,
        dcat:Resource ;
    rdfs:label "Item I88"@en-AU ;
    rdfs:comment "64 ACC  Information does not have to be reported if it has already been reported under the Migration Act 1958 - GraphNodeID: I88"@en-AU ;
    skos:definition "64 ACC  Information does not have to be reported if it has already been reported under the Migration Act 1958"@en-AU ;
    skos:narrower C1901A00006:75 ;
    skos:prefLabel "Item I88"@en-AU ;
    dcat:accessURL "https://www.legislation.gov.au/C1901A00006/2024-07-01/2024-07-01/text/original/epub/OEBPS/document_1/document_1.html#_Toc172623062"^^xsd:anyURI .

C1901A00006:880 a legcons:Division,
        skos:Concept,
        dcat:Resource ;
    rdfs:label "Division D880"@en-AU ;
    rdfs:comment "Division 4 Rules - GraphNodeID: D880"@en-AU ;
    skos:definition "Division 4 Rules"@en-AU ;
    skos:narrower C1901A00006:868 ;
    skos:prefLabel "Division D880"@en-AU ;
    dcat:accessURL "https://www.legislation.gov.au/C1901A00006/2024-07-01/2024-07-01/text/original/epub/OEBPS/document_2/document_2.html#_Toc172624635"^^xsd:anyURI .

C1901A00006:881 a legcons:Item,
        skos:Concept,
        dcat:Resource ;
    rdfs:label "Item I881"@en-AU ;
    rdfs:comment "179  Rules - GraphNodeID: I881"@en-AU ;
    skos:definition "179  Rules"@en-AU ;
    skos:narrower C1901A00006:875 ;
    skos:prefLabel "Item I881"@en-AU ;
    dcat:accessURL "https://www.legislation.gov.au/C1901A00006/2024-07-01/2024-07-01/text/original/epub/OEBPS/document_2/document_2.html#_Toc172624636"^^xsd:anyURI .

C1901A00006:883 a legcons:Division,
        skos:Concept,
        dcat:Resource ;
    rdfs:label "Division D883"@en-AU ;
    rdfs:comment "Division 1 Preliminary - GraphNodeID: D883"@en-AU ;
    skos:definition "Division 1 Preliminary"@en-AU ;
    skos:narrower C1901A00006:882 ;
    skos:prefLabel "Division D883"@en-AU ;
    dcat:accessURL "https://www.legislation.gov.au/C1901A00006/2024-07-01/2024-07-01/text/original/epub/OEBPS/document_2/document_2.html#_Toc172624638"^^xsd:anyURI .

C1901A00006:884 a legcons:Item,
        skos:Concept,
        dcat:Resource ;
    rdfs:label "Item I884"@en-AU ;
    rdfs:comment "179 A  Simplified outline of this Part - GraphNodeID: I884"@en-AU ;
    skos:definition "179 A  Simplified outline of this Part"@en-AU ;
    skos:narrower C1901A00006:875 ;
    skos:prefLabel "Item I884"@en-AU ;
    dcat:accessURL "https://www.legislation.gov.au/C1901A00006/2024-07-01/2024-07-01/text/original/epub/OEBPS/document_2/document_2.html#_Toc172624639"^^xsd:anyURI .

C1901A00006:885 a legcons:Item,
        skos:Concept,
        dcat:Resource ;
    rdfs:label "Item I885"@en-AU ;
    rdfs:comment "179 B  Application of this Part - GraphNodeID: I885"@en-AU ;
    skos:definition "179 B  Application of this Part"@en-AU ;
    skos:narrower C1901A00006:875 ;
    skos:prefLabel "Item I885"@en-AU ;
    dcat:accessURL "https://www.legislation.gov.au/C1901A00006/2024-07-01/2024-07-01/text/original/epub/OEBPS/document_2/document_2.html#_Toc172624640"^^xsd:anyURI .

C1901A00006:886 a legcons:Division,
        skos:Concept,
        dcat:Resource ;
    rdfs:label "Division D886"@en-AU ;
    rdfs:comment "Division 2 Obligations and benefits under controlled trials - GraphNodeID: D886"@en-AU ;
    skos:definition "Division 2 Obligations and benefits under controlled trials"@en-AU ;
    skos:narrower C1901A00006:882 ;
    skos:prefLabel "Division D886"@en-AU ;
    dcat:accessURL "https://www.legislation.gov.au/C1901A00006/2024-07-01/2024-07-01/text/original/epub/OEBPS/document_2/document_2.html#_Toc172624641"^^xsd:anyURI .

C1901A00006:887 a legcons:Item,
        skos:Concept,
        dcat:Resource ;
    rdfs:label "Item I887"@en-AU ;
    rdfs:comment "179 C  Obligations under controlled trials - GraphNodeID: I887"@en-AU ;
    skos:definition "179 C  Obligations under controlled trials"@en-AU ;
    skos:narrower C1901A00006:875 ;
    skos:prefLabel "Item I887"@en-AU ;
    dcat:accessURL "https://www.legislation.gov.au/C1901A00006/2024-07-01/2024-07-01/text/original/epub/OEBPS/document_2/document_2.html#_Toc172624642"^^xsd:anyURI .

C1901A00006:888 a legcons:Item,
        skos:Concept,
        dcat:Resource ;
    rdfs:label "Item I888"@en-AU ;
    rdfs:comment "179 D  Benefits under controlled trials - GraphNodeID: I888"@en-AU ;
    skos:definition "179 D  Benefits under controlled trials"@en-AU ;
    skos:narrower C1901A00006:875 ;
    skos:prefLabel "Item I888"@en-AU ;
    dcat:accessURL "https://www.legislation.gov.au/C1901A00006/2024-07-01/2024-07-01/text/original/epub/OEBPS/document_2/document_2.html#_Toc172624643"^^xsd:anyURI .

C1901A00006:889 a legcons:Division,
        skos:Concept,
        dcat:Resource ;
    rdfs:label "Division D889"@en-AU ;
    rdfs:comment "Division 3 Participation in controlled trials - GraphNodeID: D889"@en-AU ;
    skos:definition "Division 3 Participation in controlled trials"@en-AU ;
    skos:narrower C1901A00006:882 ;
    skos:prefLabel "Division D889"@en-AU ;
    dcat:accessURL "https://www.legislation.gov.au/C1901A00006/2024-07-01/2024-07-01/text/original/epub/OEBPS/document_2/document_2.html#_Toc172624644"^^xsd:anyURI .

C1901A00006:89 a legcons:Item,
        skos:Concept,
        dcat:Resource ;
    rdfs:label "Item I89"@en-AU ;
    rdfs:comment "64 ACD  Offence for failure to comply - GraphNodeID: I89"@en-AU ;
    skos:definition "64 ACD  Offence for failure to comply"@en-AU ;
    skos:narrower C1901A00006:75 ;
    skos:prefLabel "Item I89"@en-AU ;
    dcat:accessURL "https://www.legislation.gov.au/C1901A00006/2024-07-01/2024-07-01/text/original/epub/OEBPS/document_1/document_1.html#_Toc172623063"^^xsd:anyURI .

C1901A00006:890 a legcons:Item,
        skos:Concept,
        dcat:Resource ;
    rdfs:label "Item I890"@en-AU ;
    rdfs:comment "179 E  Approval of participation in controlled trials - GraphNodeID: I890"@en-AU ;
    skos:definition "179 E  Approval of participation in controlled trials"@en-AU ;
    skos:narrower C1901A00006:875 ;
    skos:prefLabel "Item I890"@en-AU ;
    dcat:accessURL "https://www.legislation.gov.au/C1901A00006/2024-07-01/2024-07-01/text/original/epub/OEBPS/document_2/document_2.html#_Toc172624645"^^xsd:anyURI .

C1901A00006:891 a legcons:Item,
        skos:Concept,
        dcat:Resource ;
    rdfs:label "Item I891"@en-AU ;
    rdfs:comment "179 F  Application to participate in controlled trial - GraphNodeID: I891"@en-AU ;
    skos:definition "179 F  Application to participate in controlled trial"@en-AU ;
    skos:narrower C1901A00006:875 ;
    skos:prefLabel "Item I891"@en-AU ;
    dcat:accessURL "https://www.legislation.gov.au/C1901A00006/2024-07-01/2024-07-01/text/original/epub/OEBPS/document_2/document_2.html#_Toc172624646"^^xsd:anyURI .

C1901A00006:892 a legcons:Item,
        skos:Concept,
        dcat:Resource ;
    rdfs:label "Item I892"@en-AU ;
    rdfs:comment "179 G  Election to participate in controlled trial - GraphNodeID: I892"@en-AU ;
    skos:definition "179 G  Election to participate in controlled trial"@en-AU ;
    skos:narrower C1901A00006:875 ;
    skos:prefLabel "Item I892"@en-AU ;
    dcat:accessURL "https://www.legislation.gov.au/C1901A00006/2024-07-01/2024-07-01/text/original/epub/OEBPS/document_2/document_2.html#_Toc172624647"^^xsd:anyURI .

C1901A00006:893 a legcons:Item,
        skos:Concept,
        dcat:Resource ;
    rdfs:label "Item I893"@en-AU ;
    rdfs:comment "179 H  Conditions of approvals - GraphNodeID: I893"@en-AU ;
    skos:definition "179 H  Conditions of approvals"@en-AU ;
    skos:narrower C1901A00006:875 ;
    skos:prefLabel "Item I893"@en-AU ;
    dcat:accessURL "https://www.legislation.gov.au/C1901A00006/2024-07-01/2024-07-01/text/original/epub/OEBPS/document_2/document_2.html#_Toc172624648"^^xsd:anyURI .

C1901A00006:894 a legcons:Item,
        skos:Concept,
        dcat:Resource ;
    rdfs:label "Item I894"@en-AU ;
    rdfs:comment "179 J  Variation suspension or revocation of approvals - GraphNodeID: I894"@en-AU ;
    skos:definition "179 J  Variation suspension or revocation of approvals"@en-AU ;
    skos:narrower C1901A00006:875 ;
    skos:prefLabel "Item I894"@en-AU ;
    dcat:accessURL "https://www.legislation.gov.au/C1901A00006/2024-07-01/2024-07-01/text/original/epub/OEBPS/document_2/document_2.html#_Toc172624649"^^xsd:anyURI .

C1901A00006:895 a legcons:Division,
        skos:Concept,
        dcat:Resource ;
    rdfs:label "Division D895"@en-AU ;
    rdfs:comment "Division 4 Instruments - GraphNodeID: D895"@en-AU ;
    skos:definition "Division 4 Instruments"@en-AU ;
    skos:narrower C1901A00006:882 ;
    skos:prefLabel "Division D895"@en-AU ;
    dcat:accessURL "https://www.legislation.gov.au/C1901A00006/2024-07-01/2024-07-01/text/original/epub/OEBPS/document_2/document_2.html#_Toc172624650"^^xsd:anyURI .

C1901A00006:896 a legcons:Item,
        skos:Concept,
        dcat:Resource ;
    rdfs:label "Item I896"@en-AU ;
    rdfs:comment "179 K  General qualification criteria for any controlled trial - GraphNodeID: I896"@en-AU ;
    skos:definition "179 K  General qualification criteria for any controlled trial"@en-AU ;
    skos:narrower C1901A00006:875 ;
    skos:prefLabel "Item I896"@en-AU ;
    dcat:accessURL "https://www.legislation.gov.au/C1901A00006/2024-07-01/2024-07-01/text/original/epub/OEBPS/document_2/document_2.html#_Toc172624651"^^xsd:anyURI .

C1901A00006:897 a legcons:Item,
        skos:Concept,
        dcat:Resource ;
    rdfs:label "Item I897"@en-AU ;
    rdfs:comment "179 L  Rules specific to a controlled trial - GraphNodeID: I897"@en-AU ;
    skos:definition "179 L  Rules specific to a controlled trial"@en-AU ;
    skos:narrower C1901A00006:875 ;
    skos:prefLabel "Item I897"@en-AU ;
    dcat:accessURL "https://www.legislation.gov.au/C1901A00006/2024-07-01/2024-07-01/text/original/epub/OEBPS/document_2/document_2.html#_Toc172624652"^^xsd:anyURI .

C1901A00006:899 a legcons:Division,
        skos:Concept,
        dcat:Resource ;
    rdfs:label "Division D899"@en-AU ;
    rdfs:comment "Division 1 Preliminary - GraphNodeID: D899"@en-AU ;
    skos:definition "Division 1 Preliminary"@en-AU ;
    skos:narrower C1901A00006:898 ;
    skos:prefLabel "Division D899"@en-AU ;
    dcat:accessURL "https://www.legislation.gov.au/C1901A00006/2024-07-01/2024-07-01/text/original/epub/OEBPS/document_2/document_2.html#_Toc172624654"^^xsd:anyURI .

C1901A00006:9 a legcons:Item,
        skos:Concept,
        dcat:Resource ;
    rdfs:label "Item I9"@en-AU ;
    rdfs:comment "4 A  Approved forms and approved statements - GraphNodeID: I9"@en-AU ;
    skos:definition "4 A  Approved forms and approved statements"@en-AU ;
    skos:narrower C1901A00006:2 ;
    skos:prefLabel "Item I9"@en-AU ;
    dcat:accessURL "https://www.legislation.gov.au/C1901A00006/2024-07-01/2024-07-01/text/original/epub/OEBPS/document_1/document_1.html#_Toc172622983"^^xsd:anyURI .

C1901A00006:90 a legcons:Item,
        skos:Concept,
        dcat:Resource ;
    rdfs:label "Item I90"@en-AU ;
    rdfs:comment "64 ACE  Communication of reports - GraphNodeID: I90"@en-AU ;
    skos:definition "64 ACE  Communication of reports"@en-AU ;
    skos:narrower C1901A00006:75 ;
    skos:prefLabel "Item I90"@en-AU ;
    dcat:accessURL "https://www.legislation.gov.au/C1901A00006/2024-07-01/2024-07-01/text/original/epub/OEBPS/document_1/document_1.html#_Toc172623064"^^xsd:anyURI .

C1901A00006:900 a legcons:Item,
        skos:Concept,
        dcat:Resource ;
    rdfs:label "Item I900"@en-AU ;
    rdfs:comment "180  Interpretation - GraphNodeID: I900"@en-AU ;
    skos:definition "180  Interpretation"@en-AU ;
    skos:narrower C1901A00006:875 ;
    skos:prefLabel "Item I900"@en-AU ;
    dcat:accessURL "https://www.legislation.gov.au/C1901A00006/2024-07-01/2024-07-01/text/original/epub/OEBPS/document_2/document_2.html#_Toc172624655"^^xsd:anyURI .

C1901A00006:901 a legcons:Division,
        skos:Concept,
        dcat:Resource ;
    rdfs:label "Division D901"@en-AU ;
    rdfs:comment "Division 2 Rights and liabilities of agents - GraphNodeID: D901"@en-AU ;
    skos:definition "Division 2 Rights and liabilities of agents"@en-AU ;
    skos:narrower C1901A00006:898 ;
    skos:prefLabel "Division D901"@en-AU ;
    dcat:accessURL "https://www.legislation.gov.au/C1901A00006/2024-07-01/2024-07-01/text/original/epub/OEBPS/document_2/document_2.html#_Toc172624656"^^xsd:anyURI .

C1901A00006:902 a legcons:Item,
        skos:Concept,
        dcat:Resource ;
    rdfs:label "Item I902"@en-AU ;
    rdfs:comment "181  Authorised agents - GraphNodeID: I902"@en-AU ;
    skos:definition "181  Authorised agents"@en-AU ;
    skos:narrower C1901A00006:875 ;
    skos:prefLabel "Item I902"@en-AU ;
    dcat:accessURL "https://www.legislation.gov.au/C1901A00006/2024-07-01/2024-07-01/text/original/epub/OEBPS/document_2/document_2.html#_Toc172624657"^^xsd:anyURI .

C1901A00006:903 a legcons:Item,
        skos:Concept,
        dcat:Resource ;
    rdfs:label "Item I903"@en-AU ;
    rdfs:comment "182  Authority to be produced - GraphNodeID: I903"@en-AU ;
    skos:definition "182  Authority to be produced"@en-AU ;
    skos:narrower C1901A00006:875 ;
    skos:prefLabel "Item I903"@en-AU ;
    dcat:accessURL "https://www.legislation.gov.au/C1901A00006/2024-07-01/2024-07-01/text/original/epub/OEBPS/document_2/document_2.html#_Toc172624658"^^xsd:anyURI .

C1901A00006:904 a legcons:Item,
        skos:Concept,
        dcat:Resource ;
    rdfs:label "Item I904"@en-AU ;
    rdfs:comment "183  Agents personally liable - GraphNodeID: I904"@en-AU ;
    skos:definition "183  Agents personally liable"@en-AU ;
    skos:narrower C1901A00006:875 ;
    skos:prefLabel "Item I904"@en-AU ;
    dcat:accessURL "https://www.legislation.gov.au/C1901A00006/2024-07-01/2024-07-01/text/original/epub/OEBPS/document_2/document_2.html#_Toc172624659"^^xsd:anyURI .

C1901A00006:905 a legcons:Item,
        skos:Concept,
        dcat:Resource ;
    rdfs:label "Item I905"@en-AU ;
    rdfs:comment "183 A  Principal liable for agents acting - GraphNodeID: I905"@en-AU ;
    skos:definition "183 A  Principal liable for agents acting"@en-AU ;
    skos:narrower C1901A00006:875 ;
    skos:prefLabel "Item I905"@en-AU ;
    dcat:accessURL "https://www.legislation.gov.au/C1901A00006/2024-07-01/2024-07-01/text/original/epub/OEBPS/document_2/document_2.html#_Toc172624660"^^xsd:anyURI .

C1901A00006:906 a legcons:Division,
        skos:Concept,
        dcat:Resource ;
    rdfs:label "Division D906"@en-AU ;
    rdfs:comment "Division 3 Licensing of customs brokers - GraphNodeID: D906"@en-AU ;
    skos:definition "Division 3 Licensing of customs brokers"@en-AU ;
    skos:narrower C1901A00006:898 ;
    skos:prefLabel "Division D906"@en-AU ;
    dcat:accessURL "https://www.legislation.gov.au/C1901A00006/2024-07-01/2024-07-01/text/original/epub/OEBPS/document_2/document_2.html#_Toc172624661"^^xsd:anyURI .

C1901A00006:907 a legcons:Item,
        skos:Concept,
        dcat:Resource ;
    rdfs:label "Item I907"@en-AU ;
    rdfs:comment "183 B  Interpretation - GraphNodeID: I907"@en-AU ;
    skos:definition "183 B  Interpretation"@en-AU ;
    skos:narrower C1901A00006:875 ;
    skos:prefLabel "Item I907"@en-AU ;
    dcat:accessURL "https://www.legislation.gov.au/C1901A00006/2024-07-01/2024-07-01/text/original/epub/OEBPS/document_2/document_2.html#_Toc172624662"^^xsd:anyURI .

C1901A00006:908 a legcons:Item,
        skos:Concept,
        dcat:Resource ;
    rdfs:label "Item I908"@en-AU ;
    rdfs:comment "183 C  Grant of licence - GraphNodeID: I908"@en-AU ;
    skos:definition "183 C  Grant of licence"@en-AU ;
    skos:narrower C1901A00006:875 ;
    skos:prefLabel "Item I908"@en-AU ;
    dcat:accessURL "https://www.legislation.gov.au/C1901A00006/2024-07-01/2024-07-01/text/original/epub/OEBPS/document_2/document_2.html#_Toc172624663"^^xsd:anyURI .

C1901A00006:909 a legcons:Item,
        skos:Concept,
        dcat:Resource ;
    rdfs:label "Item I909"@en-AU ;
    rdfs:comment "183 CA  Application for licence - GraphNodeID: I909"@en-AU ;
    skos:definition "183 CA  Application for licence"@en-AU ;
    skos:narrower C1901A00006:875 ;
    skos:prefLabel "Item I909"@en-AU ;
    dcat:accessURL "https://www.legislation.gov.au/C1901A00006/2024-07-01/2024-07-01/text/original/epub/OEBPS/document_2/document_2.html#_Toc172624664"^^xsd:anyURI .

C1901A00006:91 a legcons:Item,
        skos:Concept,
        dcat:Resource ;
    rdfs:label "Item I91"@en-AU ;
    rdfs:comment "64 ADAA  Requirements for communicating to Department electronically - GraphNodeID: I91"@en-AU ;
    skos:definition "64 ADAA  Requirements for communicating to Department electronically"@en-AU ;
    skos:narrower C1901A00006:75 ;
    skos:prefLabel "Item I91"@en-AU ;
    dcat:accessURL "https://www.legislation.gov.au/C1901A00006/2024-07-01/2024-07-01/text/original/epub/OEBPS/document_1/document_1.html#_Toc172623065"^^xsd:anyURI .

C1901A00006:910 a legcons:Item,
        skos:Concept,
        dcat:Resource ;
    rdfs:label "Item I910"@en-AU ;
    rdfs:comment "183 CB  Reference of application to Committee - GraphNodeID: I910"@en-AU ;
    skos:definition "183 CB  Reference of application to Committee"@en-AU ;
    skos:narrower C1901A00006:875 ;
    skos:prefLabel "Item I910"@en-AU ;
    dcat:accessURL "https://www.legislation.gov.au/C1901A00006/2024-07-01/2024-07-01/text/original/epub/OEBPS/document_2/document_2.html#_Toc172624665"^^xsd:anyURI .

C1901A00006:911 a legcons:Item,
        skos:Concept,
        dcat:Resource ;
    rdfs:label "Item I911"@en-AU ;
    rdfs:comment "183 CC  Requirements for grant of licence - GraphNodeID: I911"@en-AU ;
    skos:definition "183 CC  Requirements for grant of licence"@en-AU ;
    skos:narrower C1901A00006:875 ;
    skos:prefLabel "Item I911"@en-AU ;
    dcat:accessURL "https://www.legislation.gov.au/C1901A00006/2024-07-01/2024-07-01/text/original/epub/OEBPS/document_2/document_2.html#_Toc172624666"^^xsd:anyURI .

C1901A00006:912 a legcons:Item,
        skos:Concept,
        dcat:Resource ;
    rdfs:label "Item I912"@en-AU ;
    rdfs:comment "183 CD  Eligibility to be nominee - GraphNodeID: I912"@en-AU ;
    skos:definition "183 CD  Eligibility to be nominee"@en-AU ;
    skos:narrower C1901A00006:875 ;
    skos:prefLabel "Item I912"@en-AU ;
    dcat:accessURL "https://www.legislation.gov.au/C1901A00006/2024-07-01/2024-07-01/text/original/epub/OEBPS/document_2/document_2.html#_Toc172624667"^^xsd:anyURI .

C1901A00006:913 a legcons:Item,
        skos:Concept,
        dcat:Resource ;
    rdfs:label "Item I913"@en-AU ;
    rdfs:comment "183 CE  Original endorsement on licence - GraphNodeID: I913"@en-AU ;
    skos:definition "183 CE  Original endorsement on licence"@en-AU ;
    skos:narrower C1901A00006:875 ;
    skos:prefLabel "Item I913"@en-AU ;
    dcat:accessURL "https://www.legislation.gov.au/C1901A00006/2024-07-01/2024-07-01/text/original/epub/OEBPS/document_2/document_2.html#_Toc172624668"^^xsd:anyURI .

C1901A00006:914 a legcons:Item,
        skos:Concept,
        dcat:Resource ;
    rdfs:label "Item I914"@en-AU ;
    rdfs:comment "183 CF  Variation of licences - GraphNodeID: I914"@en-AU ;
    skos:definition "183 CF  Variation of licences"@en-AU ;
    skos:narrower C1901A00006:875 ;
    skos:prefLabel "Item I914"@en-AU ;
    dcat:accessURL "https://www.legislation.gov.au/C1901A00006/2024-07-01/2024-07-01/text/original/epub/OEBPS/document_2/document_2.html#_Toc172624669"^^xsd:anyURI .

C1901A00006:915 a legcons:Item,
        skos:Concept,
        dcat:Resource ;
    rdfs:label "Item I915"@en-AU ;
    rdfs:comment "183 CG  Licence granted subject to conditions - GraphNodeID: I915"@en-AU ;
    skos:definition "183 CG  Licence granted subject to conditions"@en-AU ;
    skos:narrower C1901A00006:875 ;
    skos:prefLabel "Item I915"@en-AU ;
    dcat:accessURL "https://www.legislation.gov.au/C1901A00006/2024-07-01/2024-07-01/text/original/epub/OEBPS/document_2/document_2.html#_Toc172624670"^^xsd:anyURI .

C1901A00006:916 a legcons:Item,
        skos:Concept,
        dcat:Resource ;
    rdfs:label "Item I916"@en-AU ;
    rdfs:comment "183 CGA  Comptroller General of Customs may impose additional conditions to which a brokers licence is subject - GraphNodeID: I916"@en-AU ;
    skos:definition "183 CGA  Comptroller General of Customs may impose additional conditions to which a brokers licence is subject"@en-AU ;
    skos:narrower C1901A00006:875 ;
    skos:prefLabel "Item I916"@en-AU ;
    dcat:accessURL "https://www.legislation.gov.au/C1901A00006/2024-07-01/2024-07-01/text/original/epub/OEBPS/document_2/document_2.html#_Toc172624671"^^xsd:anyURI .

C1901A00006:917 a legcons:Item,
        skos:Concept,
        dcat:Resource ;
    rdfs:label "Item I917"@en-AU ;
    rdfs:comment "183 CGB  Comptroller General of Customs may vary the conditions to which a brokers licence is subject - GraphNodeID: I917"@en-AU ;
    skos:definition "183 CGB  Comptroller General of Customs may vary the conditions to which a brokers licence is subject"@en-AU ;
    skos:narrower C1901A00006:875 ;
    skos:prefLabel "Item I917"@en-AU ;
    dcat:accessURL "https://www.legislation.gov.au/C1901A00006/2024-07-01/2024-07-01/text/original/epub/OEBPS/document_2/document_2.html#_Toc172624672"^^xsd:anyURI .

C1901A00006:918 a legcons:Item,
        skos:Concept,
        dcat:Resource ;
    rdfs:label "Item I918"@en-AU ;
    rdfs:comment "183 CGC  Breach of conditions of a brokers licence - GraphNodeID: I918"@en-AU ;
    skos:definition "183 CGC  Breach of conditions of a brokers licence"@en-AU ;
    skos:narrower C1901A00006:875 ;
    skos:prefLabel "Item I918"@en-AU ;
    dcat:accessURL "https://www.legislation.gov.au/C1901A00006/2024-07-01/2024-07-01/text/original/epub/OEBPS/document_2/document_2.html#_Toc172624673"^^xsd:anyURI .

C1901A00006:919 a legcons:Item,
        skos:Concept,
        dcat:Resource ;
    rdfs:label "Item I919"@en-AU ;
    rdfs:comment "183 CH  Duration of licence - GraphNodeID: I919"@en-AU ;
    skos:definition "183 CH  Duration of licence"@en-AU ;
    skos:narrower C1901A00006:875 ;
    skos:prefLabel "Item I919"@en-AU ;
    dcat:accessURL "https://www.legislation.gov.au/C1901A00006/2024-07-01/2024-07-01/text/original/epub/OEBPS/document_2/document_2.html#_Toc172624674"^^xsd:anyURI .

C1901A00006:92 a legcons:Item,
        skos:Concept,
        dcat:Resource ;
    rdfs:label "Item I92"@en-AU ;
    rdfs:comment "64 ADA  Disclosure of cargo reports to port authorities - GraphNodeID: I92"@en-AU ;
    skos:definition "64 ADA  Disclosure of cargo reports to port authorities"@en-AU ;
    skos:narrower C1901A00006:75 ;
    skos:prefLabel "Item I92"@en-AU ;
    dcat:accessURL "https://www.legislation.gov.au/C1901A00006/2024-07-01/2024-07-01/text/original/epub/OEBPS/document_1/document_1.html#_Toc172623066"^^xsd:anyURI .

C1901A00006:920 a legcons:Item,
        skos:Concept,
        dcat:Resource ;
    rdfs:label "Item I920"@en-AU ;
    rdfs:comment "183 CJ  Renewal of licence - GraphNodeID: I920"@en-AU ;
    skos:definition "183 CJ  Renewal of licence"@en-AU ;
    skos:narrower C1901A00006:875 ;
    skos:prefLabel "Item I920"@en-AU ;
    dcat:accessURL "https://www.legislation.gov.au/C1901A00006/2024-07-01/2024-07-01/text/original/epub/OEBPS/document_2/document_2.html#_Toc172624675"^^xsd:anyURI .

C1901A00006:921 a legcons:Item,
        skos:Concept,
        dcat:Resource ;
    rdfs:label "Item I921"@en-AU ;
    rdfs:comment "183 CJA  Licence charges - GraphNodeID: I921"@en-AU ;
    skos:definition "183 CJA  Licence charges"@en-AU ;
    skos:narrower C1901A00006:875 ;
    skos:prefLabel "Item I921"@en-AU ;
    dcat:accessURL "https://www.legislation.gov.au/C1901A00006/2024-07-01/2024-07-01/text/original/epub/OEBPS/document_2/document_2.html#_Toc172624676"^^xsd:anyURI .

C1901A00006:922 a legcons:Item,
        skos:Concept,
        dcat:Resource ;
    rdfs:label "Item I922"@en-AU ;
    rdfs:comment "183 CK  Security - GraphNodeID: I922"@en-AU ;
    skos:definition "183 CK  Security"@en-AU ;
    skos:narrower C1901A00006:875 ;
    skos:prefLabel "Item I922"@en-AU ;
    dcat:accessURL "https://www.legislation.gov.au/C1901A00006/2024-07-01/2024-07-01/text/original/epub/OEBPS/document_2/document_2.html#_Toc172624677"^^xsd:anyURI .

C1901A00006:923 a legcons:Item,
        skos:Concept,
        dcat:Resource ;
    rdfs:label "Item I923"@en-AU ;
    rdfs:comment "183 CM  Nominees - GraphNodeID: I923"@en-AU ;
    skos:definition "183 CM  Nominees"@en-AU ;
    skos:narrower C1901A00006:875 ;
    skos:prefLabel "Item I923"@en-AU ;
    dcat:accessURL "https://www.legislation.gov.au/C1901A00006/2024-07-01/2024-07-01/text/original/epub/OEBPS/document_2/document_2.html#_Toc172624678"^^xsd:anyURI .

C1901A00006:924 a legcons:Item,
        skos:Concept,
        dcat:Resource ;
    rdfs:label "Item I924"@en-AU ;
    rdfs:comment "183 CN  Removal of nominee - GraphNodeID: I924"@en-AU ;
    skos:definition "183 CN  Removal of nominee"@en-AU ;
    skos:narrower C1901A00006:875 ;
    skos:prefLabel "Item I924"@en-AU ;
    dcat:accessURL "https://www.legislation.gov.au/C1901A00006/2024-07-01/2024-07-01/text/original/epub/OEBPS/document_2/document_2.html#_Toc172624679"^^xsd:anyURI .

C1901A00006:925 a legcons:Item,
        skos:Concept,
        dcat:Resource ;
    rdfs:label "Item I925"@en-AU ;
    rdfs:comment "183 CP  Notice to nominate new nominee - GraphNodeID: I925"@en-AU ;
    skos:definition "183 CP  Notice to nominate new nominee"@en-AU ;
    skos:narrower C1901A00006:875 ;
    skos:prefLabel "Item I925"@en-AU ;
    dcat:accessURL "https://www.legislation.gov.au/C1901A00006/2024-07-01/2024-07-01/text/original/epub/OEBPS/document_2/document_2.html#_Toc172624680"^^xsd:anyURI .

C1901A00006:926 a legcons:Division,
        skos:Concept,
        dcat:Resource ;
    rdfs:label "Division D926"@en-AU ;
    rdfs:comment "Division 4 Suspension revocation and non renewal of licences - GraphNodeID: D926"@en-AU ;
    skos:definition "Division 4 Suspension revocation and non renewal of licences"@en-AU ;
    skos:narrower C1901A00006:898 ;
    skos:prefLabel "Division D926"@en-AU ;
    dcat:accessURL "https://www.legislation.gov.au/C1901A00006/2024-07-01/2024-07-01/text/original/epub/OEBPS/document_2/document_2.html#_Toc172624681"^^xsd:anyURI .

C1901A00006:927 a legcons:Item,
        skos:Concept,
        dcat:Resource ;
    rdfs:label "Item I927"@en-AU ;
    rdfs:comment "183 CQ  Investigation of matters relating to a brokers licence - GraphNodeID: I927"@en-AU ;
    skos:definition "183 CQ  Investigation of matters relating to a brokers licence"@en-AU ;
    skos:narrower C1901A00006:875 ;
    skos:prefLabel "Item I927"@en-AU ;
    dcat:accessURL "https://www.legislation.gov.au/C1901A00006/2024-07-01/2024-07-01/text/original/epub/OEBPS/document_2/document_2.html#_Toc172624682"^^xsd:anyURI .

C1901A00006:928 a legcons:Item,
        skos:Concept,
        dcat:Resource ;
    rdfs:label "Item I928"@en-AU ;
    rdfs:comment "183 CR  Interim suspension by Comptroller General of Customs - GraphNodeID: I928"@en-AU ;
    skos:definition "183 CR  Interim suspension by Comptroller General of Customs"@en-AU ;
    skos:narrower C1901A00006:875 ;
    skos:prefLabel "Item I928"@en-AU ;
    dcat:accessURL "https://www.legislation.gov.au/C1901A00006/2024-07-01/2024-07-01/text/original/epub/OEBPS/document_2/document_2.html#_Toc172624683"^^xsd:anyURI .

C1901A00006:929 a legcons:Item,
        skos:Concept,
        dcat:Resource ;
    rdfs:label "Item I929"@en-AU ;
    rdfs:comment "183 CS  Powers of Comptroller General of Customs - GraphNodeID: I929"@en-AU ;
    skos:definition "183 CS  Powers of Comptroller General of Customs"@en-AU ;
    skos:narrower C1901A00006:875 ;
    skos:prefLabel "Item I929"@en-AU ;
    dcat:accessURL "https://www.legislation.gov.au/C1901A00006/2024-07-01/2024-07-01/text/original/epub/OEBPS/document_2/document_2.html#_Toc172624684"^^xsd:anyURI .

C1901A00006:93 a legcons:Item,
        skos:Concept,
        dcat:Resource ;
    rdfs:label "Item I93"@en-AU ;
    rdfs:comment "64 AE  Obligation to answer questions and produce documents - GraphNodeID: I93"@en-AU ;
    skos:definition "64 AE  Obligation to answer questions and produce documents"@en-AU ;
    skos:narrower C1901A00006:75 ;
    skos:prefLabel "Item I93"@en-AU ;
    dcat:accessURL "https://www.legislation.gov.au/C1901A00006/2024-07-01/2024-07-01/text/original/epub/OEBPS/document_1/document_1.html#_Toc172623067"^^xsd:anyURI .

C1901A00006:930 a legcons:Item,
        skos:Concept,
        dcat:Resource ;
    rdfs:label "Item I930"@en-AU ;
    rdfs:comment "183 CT  Effect of suspension - GraphNodeID: I930"@en-AU ;
    skos:definition "183 CT  Effect of suspension"@en-AU ;
    skos:narrower C1901A00006:875 ;
    skos:prefLabel "Item I930"@en-AU ;
    dcat:accessURL "https://www.legislation.gov.au/C1901A00006/2024-07-01/2024-07-01/text/original/epub/OEBPS/document_2/document_2.html#_Toc172624685"^^xsd:anyURI .

C1901A00006:931 a legcons:Item,
        skos:Concept,
        dcat:Resource ;
    rdfs:label "Item I931"@en-AU ;
    rdfs:comment "183 CU  Service of notices - GraphNodeID: I931"@en-AU ;
    skos:definition "183 CU  Service of notices"@en-AU ;
    skos:narrower C1901A00006:875 ;
    skos:prefLabel "Item I931"@en-AU ;
    dcat:accessURL "https://www.legislation.gov.au/C1901A00006/2024-07-01/2024-07-01/text/original/epub/OEBPS/document_2/document_2.html#_Toc172624686"^^xsd:anyURI .

C1901A00006:932 a legcons:Division,
        skos:Concept,
        dcat:Resource ;
    rdfs:label "Division D932"@en-AU ;
    rdfs:comment "Division 5 National Customs Brokers Licensing Advisory Committee - GraphNodeID: D932"@en-AU ;
    skos:definition "Division 5 National Customs Brokers Licensing Advisory Committee"@en-AU ;
    skos:narrower C1901A00006:898 ;
    skos:prefLabel "Division D932"@en-AU ;
    dcat:accessURL "https://www.legislation.gov.au/C1901A00006/2024-07-01/2024-07-01/text/original/epub/OEBPS/document_2/document_2.html#_Toc172624687"^^xsd:anyURI .

C1901A00006:933 a legcons:Item,
        skos:Concept,
        dcat:Resource ;
    rdfs:label "Item I933"@en-AU ;
    rdfs:comment "183 D  National Customs Brokers Licensing Advisory Committee - GraphNodeID: I933"@en-AU ;
    skos:definition "183 D  National Customs Brokers Licensing Advisory Committee"@en-AU ;
    skos:narrower C1901A00006:875 ;
    skos:prefLabel "Item I933"@en-AU ;
    dcat:accessURL "https://www.legislation.gov.au/C1901A00006/2024-07-01/2024-07-01/text/original/epub/OEBPS/document_2/document_2.html#_Toc172624688"^^xsd:anyURI .

C1901A00006:934 a legcons:Item,
        skos:Concept,
        dcat:Resource ;
    rdfs:label "Item I934"@en-AU ;
    rdfs:comment "183 DA  Constitution of Committee - GraphNodeID: I934"@en-AU ;
    skos:definition "183 DA  Constitution of Committee"@en-AU ;
    skos:narrower C1901A00006:875 ;
    skos:prefLabel "Item I934"@en-AU ;
    dcat:accessURL "https://www.legislation.gov.au/C1901A00006/2024-07-01/2024-07-01/text/original/epub/OEBPS/document_2/document_2.html#_Toc172624689"^^xsd:anyURI .

C1901A00006:935 a legcons:Item,
        skos:Concept,
        dcat:Resource ;
    rdfs:label "Item I935"@en-AU ;
    rdfs:comment "183 DB  Remuneration and allowances - GraphNodeID: I935"@en-AU ;
    skos:definition "183 DB  Remuneration and allowances"@en-AU ;
    skos:narrower C1901A00006:875 ;
    skos:prefLabel "Item I935"@en-AU ;
    dcat:accessURL "https://www.legislation.gov.au/C1901A00006/2024-07-01/2024-07-01/text/original/epub/OEBPS/document_2/document_2.html#_Toc172624690"^^xsd:anyURI .

C1901A00006:936 a legcons:Item,
        skos:Concept,
        dcat:Resource ;
    rdfs:label "Item I936"@en-AU ;
    rdfs:comment "183 DC  Acting Chair - GraphNodeID: I936"@en-AU ;
    skos:definition "183 DC  Acting Chair"@en-AU ;
    skos:narrower C1901A00006:875 ;
    skos:prefLabel "Item I936"@en-AU ;
    dcat:accessURL "https://www.legislation.gov.au/C1901A00006/2024-07-01/2024-07-01/text/original/epub/OEBPS/document_2/document_2.html#_Toc172624691"^^xsd:anyURI .

C1901A00006:937 a legcons:Item,
        skos:Concept,
        dcat:Resource ;
    rdfs:label "Item I937"@en-AU ;
    rdfs:comment "183 DD  Deputy member - GraphNodeID: I937"@en-AU ;
    skos:definition "183 DD  Deputy member"@en-AU ;
    skos:narrower C1901A00006:875 ;
    skos:prefLabel "Item I937"@en-AU ;
    dcat:accessURL "https://www.legislation.gov.au/C1901A00006/2024-07-01/2024-07-01/text/original/epub/OEBPS/document_2/document_2.html#_Toc172624692"^^xsd:anyURI .

C1901A00006:938 a legcons:Item,
        skos:Concept,
        dcat:Resource ;
    rdfs:label "Item I938"@en-AU ;
    rdfs:comment "183 E  Procedure of Committees - GraphNodeID: I938"@en-AU ;
    skos:definition "183 E  Procedure of Committees"@en-AU ;
    skos:narrower C1901A00006:875 ;
    skos:prefLabel "Item I938"@en-AU ;
    dcat:accessURL "https://www.legislation.gov.au/C1901A00006/2024-07-01/2024-07-01/text/original/epub/OEBPS/document_2/document_2.html#_Toc172624693"^^xsd:anyURI .

C1901A00006:939 a legcons:Item,
        skos:Concept,
        dcat:Resource ;
    rdfs:label "Item I939"@en-AU ;
    rdfs:comment "183 F  Evidence - GraphNodeID: I939"@en-AU ;
    skos:definition "183 F  Evidence"@en-AU ;
    skos:narrower C1901A00006:875 ;
    skos:prefLabel "Item I939"@en-AU ;
    dcat:accessURL "https://www.legislation.gov.au/C1901A00006/2024-07-01/2024-07-01/text/original/epub/OEBPS/document_2/document_2.html#_Toc172624694"^^xsd:anyURI .

C1901A00006:94 a legcons:Item,
        skos:Concept,
        dcat:Resource ;
    rdfs:label "Item I94"@en-AU ;
    rdfs:comment "64 AF  Obligation to provide access to passenger information - GraphNodeID: I94"@en-AU ;
    skos:definition "64 AF  Obligation to provide access to passenger information"@en-AU ;
    skos:narrower C1901A00006:75 ;
    skos:prefLabel "Item I94"@en-AU ;
    dcat:accessURL "https://www.legislation.gov.au/C1901A00006/2024-07-01/2024-07-01/text/original/epub/OEBPS/document_1/document_1.html#_Toc172623068"^^xsd:anyURI .

C1901A00006:940 a legcons:Item,
        skos:Concept,
        dcat:Resource ;
    rdfs:label "Item I940"@en-AU ;
    rdfs:comment "183 G  Proceedings in private - GraphNodeID: I940"@en-AU ;
    skos:definition "183 G  Proceedings in private"@en-AU ;
    skos:narrower C1901A00006:875 ;
    skos:prefLabel "Item I940"@en-AU ;
    dcat:accessURL "https://www.legislation.gov.au/C1901A00006/2024-07-01/2024-07-01/text/original/epub/OEBPS/document_2/document_2.html#_Toc172624695"^^xsd:anyURI .

C1901A00006:941 a legcons:Item,
        skos:Concept,
        dcat:Resource ;
    rdfs:label "Item I941"@en-AU ;
    rdfs:comment "183 H  Determination of questions before a Committee - GraphNodeID: I941"@en-AU ;
    skos:definition "183 H  Determination of questions before a Committee"@en-AU ;
    skos:narrower C1901A00006:875 ;
    skos:prefLabel "Item I941"@en-AU ;
    dcat:accessURL "https://www.legislation.gov.au/C1901A00006/2024-07-01/2024-07-01/text/original/epub/OEBPS/document_2/document_2.html#_Toc172624696"^^xsd:anyURI .

C1901A00006:942 a legcons:Item,
        skos:Concept,
        dcat:Resource ;
    rdfs:label "Item I942"@en-AU ;
    rdfs:comment "183 J  Customs broker affected by investigations to be given notice - GraphNodeID: I942"@en-AU ;
    skos:definition "183 J  Customs broker affected by investigations to be given notice"@en-AU ;
    skos:narrower C1901A00006:875 ;
    skos:prefLabel "Item I942"@en-AU ;
    dcat:accessURL "https://www.legislation.gov.au/C1901A00006/2024-07-01/2024-07-01/text/original/epub/OEBPS/document_2/document_2.html#_Toc172624697"^^xsd:anyURI .

C1901A00006:943 a legcons:Item,
        skos:Concept,
        dcat:Resource ;
    rdfs:label "Item I943"@en-AU ;
    rdfs:comment "183 K  Summoning of witnesses - GraphNodeID: I943"@en-AU ;
    skos:definition "183 K  Summoning of witnesses"@en-AU ;
    skos:narrower C1901A00006:875 ;
    skos:prefLabel "Item I943"@en-AU ;
    dcat:accessURL "https://www.legislation.gov.au/C1901A00006/2024-07-01/2024-07-01/text/original/epub/OEBPS/document_2/document_2.html#_Toc172624698"^^xsd:anyURI .

C1901A00006:944 a legcons:Item,
        skos:Concept,
        dcat:Resource ;
    rdfs:label "Item I944"@en-AU ;
    rdfs:comment "183 L  Service of notices and summonses - GraphNodeID: I944"@en-AU ;
    skos:definition "183 L  Service of notices and summonses"@en-AU ;
    skos:narrower C1901A00006:875 ;
    skos:prefLabel "Item I944"@en-AU ;
    dcat:accessURL "https://www.legislation.gov.au/C1901A00006/2024-07-01/2024-07-01/text/original/epub/OEBPS/document_2/document_2.html#_Toc172624699"^^xsd:anyURI .

C1901A00006:945 a legcons:Item,
        skos:Concept,
        dcat:Resource ;
    rdfs:label "Item I945"@en-AU ;
    rdfs:comment "183 N  Committee may examine upon oath or affirmation - GraphNodeID: I945"@en-AU ;
    skos:definition "183 N  Committee may examine upon oath or affirmation"@en-AU ;
    skos:narrower C1901A00006:875 ;
    skos:prefLabel "Item I945"@en-AU ;
    dcat:accessURL "https://www.legislation.gov.au/C1901A00006/2024-07-01/2024-07-01/text/original/epub/OEBPS/document_2/document_2.html#_Toc172624700"^^xsd:anyURI .

C1901A00006:946 a legcons:Item,
        skos:Concept,
        dcat:Resource ;
    rdfs:label "Item I946"@en-AU ;
    rdfs:comment "183 P  Offences by witness - GraphNodeID: I946"@en-AU ;
    skos:definition "183 P  Offences by witness"@en-AU ;
    skos:narrower C1901A00006:875 ;
    skos:prefLabel "Item I946"@en-AU ;
    dcat:accessURL "https://www.legislation.gov.au/C1901A00006/2024-07-01/2024-07-01/text/original/epub/OEBPS/document_2/document_2.html#_Toc172624701"^^xsd:anyURI .

C1901A00006:947 a legcons:Item,
        skos:Concept,
        dcat:Resource ;
    rdfs:label "Item I947"@en-AU ;
    rdfs:comment "183 Q  Statements by witness - GraphNodeID: I947"@en-AU ;
    skos:definition "183 Q  Statements by witness"@en-AU ;
    skos:narrower C1901A00006:875 ;
    skos:prefLabel "Item I947"@en-AU ;
    dcat:accessURL "https://www.legislation.gov.au/C1901A00006/2024-07-01/2024-07-01/text/original/epub/OEBPS/document_2/document_2.html#_Toc172624702"^^xsd:anyURI .

C1901A00006:948 a legcons:Item,
        skos:Concept,
        dcat:Resource ;
    rdfs:label "Item I948"@en-AU ;
    rdfs:comment "183 R  Witness fees - GraphNodeID: I948"@en-AU ;
    skos:definition "183 R  Witness fees"@en-AU ;
    skos:narrower C1901A00006:875 ;
    skos:prefLabel "Item I948"@en-AU ;
    dcat:accessURL "https://www.legislation.gov.au/C1901A00006/2024-07-01/2024-07-01/text/original/epub/OEBPS/document_2/document_2.html#_Toc172624703"^^xsd:anyURI .

C1901A00006:949 a legcons:Item,
        skos:Concept,
        dcat:Resource ;
    rdfs:label "Item I949"@en-AU ;
    rdfs:comment "183 S  Representation by counsel etc - GraphNodeID: I949"@en-AU ;
    skos:definition "183 S  Representation by counsel etc"@en-AU ;
    skos:narrower C1901A00006:875 ;
    skos:prefLabel "Item I949"@en-AU ;
    dcat:accessURL "https://www.legislation.gov.au/C1901A00006/2024-07-01/2024-07-01/text/original/epub/OEBPS/document_2/document_2.html#_Toc172624704"^^xsd:anyURI .

C1901A00006:95 a legcons:Item,
        skos:Concept,
        dcat:Resource ;
    rdfs:label "Item I95"@en-AU ;
    rdfs:comment "64 A  Ships or aircraft arriving at certain places - GraphNodeID: I95"@en-AU ;
    skos:definition "64 A  Ships or aircraft arriving at certain places"@en-AU ;
    skos:narrower C1901A00006:75 ;
    skos:prefLabel "Item I95"@en-AU ;
    dcat:accessURL "https://www.legislation.gov.au/C1901A00006/2024-07-01/2024-07-01/text/original/epub/OEBPS/document_1/document_1.html#_Toc172623069"^^xsd:anyURI .

C1901A00006:950 a legcons:Item,
        skos:Concept,
        dcat:Resource ;
    rdfs:label "Item I950"@en-AU ;
    rdfs:comment "183 T  Protection of members - GraphNodeID: I950"@en-AU ;
    skos:definition "183 T  Protection of members"@en-AU ;
    skos:narrower C1901A00006:875 ;
    skos:prefLabel "Item I950"@en-AU ;
    dcat:accessURL "https://www.legislation.gov.au/C1901A00006/2024-07-01/2024-07-01/text/original/epub/OEBPS/document_2/document_2.html#_Toc172624705"^^xsd:anyURI .

C1901A00006:951 a legcons:Item,
        skos:Concept,
        dcat:Resource ;
    rdfs:label "Item I951"@en-AU ;
    rdfs:comment "183 U  Protection of barristers witnesses etc - GraphNodeID: I951"@en-AU ;
    skos:definition "183 U  Protection of barristers witnesses etc"@en-AU ;
    skos:narrower C1901A00006:875 ;
    skos:prefLabel "Item I951"@en-AU ;
    dcat:accessURL "https://www.legislation.gov.au/C1901A00006/2024-07-01/2024-07-01/text/original/epub/OEBPS/document_2/document_2.html#_Toc172624706"^^xsd:anyURI .

C1901A00006:956 a legcons:Item,
        skos:Concept,
        dcat:Resource ;
    rdfs:label "Item I956"@en-AU ;
    rdfs:comment "183 UA  Definitions - GraphNodeID: I956"@en-AU ;
    skos:definition "183 UA  Definitions"@en-AU ;
    skos:narrower C1901A00006:955 ;
    skos:prefLabel "Item I956"@en-AU ;
    dcat:accessURL "https://www.legislation.gov.au/C1901A00006/2024-07-01/2024-07-01/text/original/epub/OEBPS/document_3/document_3.html#_Toc172626990"^^xsd:anyURI .

C1901A00006:957 a legcons:Item,
        skos:Concept,
        dcat:Resource ;
    rdfs:label "Item I957"@en-AU ;
    rdfs:comment "183 UB  Law relating to legal professional privilege not affected - GraphNodeID: I957"@en-AU ;
    skos:definition "183 UB  Law relating to legal professional privilege not affected"@en-AU ;
    skos:narrower C1901A00006:955 ;
    skos:prefLabel "Item I957"@en-AU ;
    dcat:accessURL "https://www.legislation.gov.au/C1901A00006/2024-07-01/2024-07-01/text/original/epub/OEBPS/document_3/document_3.html#_Toc172626991"^^xsd:anyURI .

C1901A00006:958 a legcons:Item,
        skos:Concept,
        dcat:Resource ;
    rdfs:label "Item I958"@en-AU ;
    rdfs:comment "183 UC  Comptroller General of Customs may give directions concerning the exercise of powers under this Division - GraphNodeID: I958"@en-AU ;
    skos:definition "183 UC  Comptroller General of Customs may give directions concerning the exercise of powers under this Division"@en-AU ;
    skos:narrower C1901A00006:955 ;
    skos:prefLabel "Item I958"@en-AU ;
    dcat:accessURL "https://www.legislation.gov.au/C1901A00006/2024-07-01/2024-07-01/text/original/epub/OEBPS/document_3/document_3.html#_Toc172626992"^^xsd:anyURI .

C1901A00006:959 a legcons:Item,
        skos:Concept,
        dcat:Resource ;
    rdfs:label "Item I959"@en-AU ;
    rdfs:comment "183 UD  Judges who may issue seizure warrants for goods in transit - GraphNodeID: I959"@en-AU ;
    skos:definition "183 UD  Judges who may issue seizure warrants for goods in transit"@en-AU ;
    skos:narrower C1901A00006:955 ;
    skos:prefLabel "Item I959"@en-AU ;
    dcat:accessURL "https://www.legislation.gov.au/C1901A00006/2024-07-01/2024-07-01/text/original/epub/OEBPS/document_3/document_3.html#_Toc172626993"^^xsd:anyURI .

C1901A00006:96 a legcons:Item,
        skos:Concept,
        dcat:Resource ;
    rdfs:label "Item I96"@en-AU ;
    rdfs:comment "65  Master or pilot of wrecked ship or aircraft to report - GraphNodeID: I96"@en-AU ;
    skos:definition "65  Master or pilot of wrecked ship or aircraft to report"@en-AU ;
    skos:narrower C1901A00006:75 ;
    skos:prefLabel "Item I96"@en-AU ;
    dcat:accessURL "https://www.legislation.gov.au/C1901A00006/2024-07-01/2024-07-01/text/original/epub/OEBPS/document_1/document_1.html#_Toc172623070"^^xsd:anyURI .

C1901A00006:961 a legcons:Item,
        skos:Concept,
        dcat:Resource ;
    rdfs:label "Item I961"@en-AU ;
    rdfs:comment "186  General powers of examination of goods subject to customs control - GraphNodeID: I961"@en-AU ;
    skos:definition "186  General powers of examination of goods subject to customs control"@en-AU ;
    skos:narrower C1901A00006:960 ;
    skos:prefLabel "Item I961"@en-AU ;
    dcat:accessURL "https://www.legislation.gov.au/C1901A00006/2024-07-01/2024-07-01/text/original/epub/OEBPS/document_3/document_3.html#_Toc172626995"^^xsd:anyURI .

C1901A00006:962 a legcons:Item,
        skos:Concept,
        dcat:Resource ;
    rdfs:label "Item I962"@en-AU ;
    rdfs:comment "186 AA  General powers of examination of goods loaded onto or unloaded from ships or aircraft - GraphNodeID: I962"@en-AU ;
    skos:definition "186 AA  General powers of examination of goods loaded onto or unloaded from ships or aircraft"@en-AU ;
    skos:narrower C1901A00006:960 ;
    skos:prefLabel "Item I962"@en-AU ;
    dcat:accessURL "https://www.legislation.gov.au/C1901A00006/2024-07-01/2024-07-01/text/original/epub/OEBPS/document_3/document_3.html#_Toc172626996"^^xsd:anyURI .

C1901A00006:963 a legcons:Item,
        skos:Concept,
        dcat:Resource ;
    rdfs:label "Item I963"@en-AU ;
    rdfs:comment "186 A  Power to make copies of and take extracts from documents in certain circumstances - GraphNodeID: I963"@en-AU ;
    skos:definition "186 A  Power to make copies of and take extracts from documents in certain circumstances"@en-AU ;
    skos:narrower C1901A00006:960 ;
    skos:prefLabel "Item I963"@en-AU ;
    dcat:accessURL "https://www.legislation.gov.au/C1901A00006/2024-07-01/2024-07-01/text/original/epub/OEBPS/document_3/document_3.html#_Toc172626997"^^xsd:anyURI .

C1901A00006:964 a legcons:Item,
        skos:Concept,
        dcat:Resource ;
    rdfs:label "Item I964"@en-AU ;
    rdfs:comment "186 B  Compensation for damage caused by copying - GraphNodeID: I964"@en-AU ;
    skos:definition "186 B  Compensation for damage caused by copying"@en-AU ;
    skos:narrower C1901A00006:960 ;
    skos:prefLabel "Item I964"@en-AU ;
    dcat:accessURL "https://www.legislation.gov.au/C1901A00006/2024-07-01/2024-07-01/text/original/epub/OEBPS/document_3/document_3.html#_Toc172626998"^^xsd:anyURI .

C1901A00006:965 a legcons:Item,
        skos:Concept,
        dcat:Resource ;
    rdfs:label "Item I965"@en-AU ;
    rdfs:comment "187  Power to board and search - GraphNodeID: I965"@en-AU ;
    skos:definition "187  Power to board and search"@en-AU ;
    skos:narrower C1901A00006:960 ;
    skos:prefLabel "Item I965"@en-AU ;
    dcat:accessURL "https://www.legislation.gov.au/C1901A00006/2024-07-01/2024-07-01/text/original/epub/OEBPS/document_3/document_3.html#_Toc172626999"^^xsd:anyURI .

C1901A00006:966 a legcons:Item,
        skos:Concept,
        dcat:Resource ;
    rdfs:label "Item I966"@en-AU ;
    rdfs:comment "188  Boarding - GraphNodeID: I966"@en-AU ;
    skos:definition "188  Boarding"@en-AU ;
    skos:narrower C1901A00006:960 ;
    skos:prefLabel "Item I966"@en-AU ;
    dcat:accessURL "https://www.legislation.gov.au/C1901A00006/2024-07-01/2024-07-01/text/original/epub/OEBPS/document_3/document_3.html#_Toc172627000"^^xsd:anyURI .

C1901A00006:967 a legcons:Item,
        skos:Concept,
        dcat:Resource ;
    rdfs:label "Item I967"@en-AU ;
    rdfs:comment "189  Searching - GraphNodeID: I967"@en-AU ;
    skos:definition "189  Searching"@en-AU ;
    skos:narrower C1901A00006:960 ;
    skos:prefLabel "Item I967"@en-AU ;
    dcat:accessURL "https://www.legislation.gov.au/C1901A00006/2024-07-01/2024-07-01/text/original/epub/OEBPS/document_3/document_3.html#_Toc172627001"^^xsd:anyURI .

C1901A00006:968 a legcons:Item,
        skos:Concept,
        dcat:Resource ;
    rdfs:label "Item I968"@en-AU ;
    rdfs:comment "189 A  Officers may carry arms in certain circumstances - GraphNodeID: I968"@en-AU ;
    skos:definition "189 A  Officers may carry arms in certain circumstances"@en-AU ;
    skos:narrower C1901A00006:960 ;
    skos:prefLabel "Item I968"@en-AU ;
    dcat:accessURL "https://www.legislation.gov.au/C1901A00006/2024-07-01/2024-07-01/text/original/epub/OEBPS/document_3/document_3.html#_Toc172627002"^^xsd:anyURI .

C1901A00006:969 a legcons:Item,
        skos:Concept,
        dcat:Resource ;
    rdfs:label "Item I969"@en-AU ;
    rdfs:comment "190  Securing goods - GraphNodeID: I969"@en-AU ;
    skos:definition "190  Securing goods"@en-AU ;
    skos:narrower C1901A00006:960 ;
    skos:prefLabel "Item I969"@en-AU ;
    dcat:accessURL "https://www.legislation.gov.au/C1901A00006/2024-07-01/2024-07-01/text/original/epub/OEBPS/document_3/document_3.html#_Toc172627003"^^xsd:anyURI .

C1901A00006:97 a legcons:Item,
        skos:Concept,
        dcat:Resource ;
    rdfs:label "Item I97"@en-AU ;
    rdfs:comment "66  Goods derelict to be delivered to officer - GraphNodeID: I97"@en-AU ;
    skos:definition "66  Goods derelict to be delivered to officer"@en-AU ;
    skos:narrower C1901A00006:75 ;
    skos:prefLabel "Item I97"@en-AU ;
    dcat:accessURL "https://www.legislation.gov.au/C1901A00006/2024-07-01/2024-07-01/text/original/epub/OEBPS/document_1/document_1.html#_Toc172623071"^^xsd:anyURI .

C1901A00006:970 a legcons:Item,
        skos:Concept,
        dcat:Resource ;
    rdfs:label "Item I970"@en-AU ;
    rdfs:comment "191  Seals etc not to be broken - GraphNodeID: I970"@en-AU ;
    skos:definition "191  Seals etc not to be broken"@en-AU ;
    skos:narrower C1901A00006:960 ;
    skos:prefLabel "Item I970"@en-AU ;
    dcat:accessURL "https://www.legislation.gov.au/C1901A00006/2024-07-01/2024-07-01/text/original/epub/OEBPS/document_3/document_3.html#_Toc172627004"^^xsd:anyURI .

C1901A00006:971 a legcons:Item,
        skos:Concept,
        dcat:Resource ;
    rdfs:label "Item I971"@en-AU ;
    rdfs:comment "192  Seals etc on ship or aircraft in port bound to another port within Commonwealth - GraphNodeID: I971"@en-AU ;
    skos:definition "192  Seals etc on ship or aircraft in port bound to another port within Commonwealth"@en-AU ;
    skos:narrower C1901A00006:960 ;
    skos:prefLabel "Item I971"@en-AU ;
    dcat:accessURL "https://www.legislation.gov.au/C1901A00006/2024-07-01/2024-07-01/text/original/epub/OEBPS/document_3/document_3.html#_Toc172627005"^^xsd:anyURI .

C1901A00006:972 a legcons:Item,
        skos:Concept,
        dcat:Resource ;
    rdfs:label "Item I972"@en-AU ;
    rdfs:comment "193  Officers may enter and remain upon coasts etc - GraphNodeID: I972"@en-AU ;
    skos:definition "193  Officers may enter and remain upon coasts etc"@en-AU ;
    skos:narrower C1901A00006:960 ;
    skos:prefLabel "Item I972"@en-AU ;
    dcat:accessURL "https://www.legislation.gov.au/C1901A00006/2024-07-01/2024-07-01/text/original/epub/OEBPS/document_3/document_3.html#_Toc172627006"^^xsd:anyURI .

C1901A00006:973 a legcons:Item,
        skos:Concept,
        dcat:Resource ;
    rdfs:label "Item I973"@en-AU ;
    rdfs:comment "194  Ships on service may be moored in any place - GraphNodeID: I973"@en-AU ;
    skos:definition "194  Ships on service may be moored in any place"@en-AU ;
    skos:narrower C1901A00006:960 ;
    skos:prefLabel "Item I973"@en-AU ;
    dcat:accessURL "https://www.legislation.gov.au/C1901A00006/2024-07-01/2024-07-01/text/original/epub/OEBPS/document_3/document_3.html#_Toc172627007"^^xsd:anyURI .

C1901A00006:974 a legcons:Item,
        skos:Concept,
        dcat:Resource ;
    rdfs:label "Item I974"@en-AU ;
    rdfs:comment "195  Power to question passengers etc - GraphNodeID: I974"@en-AU ;
    skos:definition "195  Power to question passengers etc"@en-AU ;
    skos:narrower C1901A00006:960 ;
    skos:prefLabel "Item I974"@en-AU ;
    dcat:accessURL "https://www.legislation.gov.au/C1901A00006/2024-07-01/2024-07-01/text/original/epub/OEBPS/document_3/document_3.html#_Toc172627008"^^xsd:anyURI .

C1901A00006:975 a legcons:Item,
        skos:Concept,
        dcat:Resource ;
    rdfs:label "Item I975"@en-AU ;
    rdfs:comment "195 A  Power to question persons found in restricted areas - GraphNodeID: I975"@en-AU ;
    skos:definition "195 A  Power to question persons found in restricted areas"@en-AU ;
    skos:narrower C1901A00006:960 ;
    skos:prefLabel "Item I975"@en-AU ;
    dcat:accessURL "https://www.legislation.gov.au/C1901A00006/2024-07-01/2024-07-01/text/original/epub/OEBPS/document_3/document_3.html#_Toc172627009"^^xsd:anyURI .

C1901A00006:976 a legcons:Item,
        skos:Concept,
        dcat:Resource ;
    rdfs:label "Item I976"@en-AU ;
    rdfs:comment "196 C  Power to question persons claiming packages - GraphNodeID: I976"@en-AU ;
    skos:definition "196 C  Power to question persons claiming packages"@en-AU ;
    skos:narrower C1901A00006:960 ;
    skos:prefLabel "Item I976"@en-AU ;
    dcat:accessURL "https://www.legislation.gov.au/C1901A00006/2024-07-01/2024-07-01/text/original/epub/OEBPS/document_3/document_3.html#_Toc172627010"^^xsd:anyURI .

C1901A00006:977 a legcons:Item,
        skos:Concept,
        dcat:Resource ;
    rdfs:label "Item I977"@en-AU ;
    rdfs:comment "197  Power to stop conveyances about to leave a Customs place - GraphNodeID: I977"@en-AU ;
    skos:definition "197  Power to stop conveyances about to leave a Customs place"@en-AU ;
    skos:narrower C1901A00006:960 ;
    skos:prefLabel "Item I977"@en-AU ;
    dcat:accessURL "https://www.legislation.gov.au/C1901A00006/2024-07-01/2024-07-01/text/original/epub/OEBPS/document_3/document_3.html#_Toc172627011"^^xsd:anyURI .

C1901A00006:979 a legcons:Item,
        skos:Concept,
        dcat:Resource ;
    rdfs:label "Item I979"@en-AU ;
    rdfs:comment "198  When search warrants relating to premises can be issued - GraphNodeID: I979"@en-AU ;
    skos:definition "198  When search warrants relating to premises can be issued"@en-AU ;
    skos:narrower C1901A00006:978 ;
    skos:prefLabel "Item I979"@en-AU ;
    dcat:accessURL "https://www.legislation.gov.au/C1901A00006/2024-07-01/2024-07-01/text/original/epub/OEBPS/document_3/document_3.html#_Toc172627013"^^xsd:anyURI .

C1901A00006:98 a legcons:Item,
        skos:Concept,
        dcat:Resource ;
    rdfs:label "Item I98"@en-AU ;
    rdfs:comment "67  Interference with derelict goods - GraphNodeID: I98"@en-AU ;
    skos:definition "67  Interference with derelict goods"@en-AU ;
    skos:narrower C1901A00006:75 ;
    skos:prefLabel "Item I98"@en-AU ;
    dcat:accessURL "https://www.legislation.gov.au/C1901A00006/2024-07-01/2024-07-01/text/original/epub/OEBPS/document_1/document_1.html#_Toc172623072"^^xsd:anyURI .

C1901A00006:980 a legcons:Item,
        skos:Concept,
        dcat:Resource ;
    rdfs:label "Item I980"@en-AU ;
    rdfs:comment "199  The things that are authorised by a search warrant relating to premises - GraphNodeID: I980"@en-AU ;
    skos:definition "199  The things that are authorised by a search warrant relating to premises"@en-AU ;
    skos:narrower C1901A00006:978 ;
    skos:prefLabel "Item I980"@en-AU ;
    dcat:accessURL "https://www.legislation.gov.au/C1901A00006/2024-07-01/2024-07-01/text/original/epub/OEBPS/document_3/document_3.html#_Toc172627014"^^xsd:anyURI .

C1901A00006:981 a legcons:Item,
        skos:Concept,
        dcat:Resource ;
    rdfs:label "Item I981"@en-AU ;
    rdfs:comment "199 A  When search warrants relating to persons can be issued - GraphNodeID: I981"@en-AU ;
    skos:definition "199 A  When search warrants relating to persons can be issued"@en-AU ;
    skos:narrower C1901A00006:978 ;
    skos:prefLabel "Item I981"@en-AU ;
    dcat:accessURL "https://www.legislation.gov.au/C1901A00006/2024-07-01/2024-07-01/text/original/epub/OEBPS/document_3/document_3.html#_Toc172627015"^^xsd:anyURI .

C1901A00006:982 a legcons:Item,
        skos:Concept,
        dcat:Resource ;
    rdfs:label "Item I982"@en-AU ;
    rdfs:comment "199 B  The things that are authorised by a search warrant relating to a person - GraphNodeID: I982"@en-AU ;
    skos:definition "199 B  The things that are authorised by a search warrant relating to a person"@en-AU ;
    skos:narrower C1901A00006:978 ;
    skos:prefLabel "Item I982"@en-AU ;
    dcat:accessURL "https://www.legislation.gov.au/C1901A00006/2024-07-01/2024-07-01/text/original/epub/OEBPS/document_3/document_3.html#_Toc172627016"^^xsd:anyURI .

C1901A00006:983 a legcons:Item,
        skos:Concept,
        dcat:Resource ;
    rdfs:label "Item I983"@en-AU ;
    rdfs:comment "200  Use of equipment to examine or process things - GraphNodeID: I983"@en-AU ;
    skos:definition "200  Use of equipment to examine or process things"@en-AU ;
    skos:narrower C1901A00006:978 ;
    skos:prefLabel "Item I983"@en-AU ;
    dcat:accessURL "https://www.legislation.gov.au/C1901A00006/2024-07-01/2024-07-01/text/original/epub/OEBPS/document_3/document_3.html#_Toc172627017"^^xsd:anyURI .

C1901A00006:984 a legcons:Item,
        skos:Concept,
        dcat:Resource ;
    rdfs:label "Item I984"@en-AU ;
    rdfs:comment "201  Use of electronic equipment on or in premises - GraphNodeID: I984"@en-AU ;
    skos:definition "201  Use of electronic equipment on or in premises"@en-AU ;
    skos:narrower C1901A00006:978 ;
    skos:prefLabel "Item I984"@en-AU ;
    dcat:accessURL "https://www.legislation.gov.au/C1901A00006/2024-07-01/2024-07-01/text/original/epub/OEBPS/document_3/document_3.html#_Toc172627018"^^xsd:anyURI .

C1901A00006:985 a legcons:Item,
        skos:Concept,
        dcat:Resource ;
    rdfs:label "Item I985"@en-AU ;
    rdfs:comment "201 AA  Use of electronic equipment at other place - GraphNodeID: I985"@en-AU ;
    skos:definition "201 AA  Use of electronic equipment at other place"@en-AU ;
    skos:narrower C1901A00006:978 ;
    skos:prefLabel "Item I985"@en-AU ;
    dcat:accessURL "https://www.legislation.gov.au/C1901A00006/2024-07-01/2024-07-01/text/original/epub/OEBPS/document_3/document_3.html#_Toc172627019"^^xsd:anyURI .

C1901A00006:986 a legcons:Item,
        skos:Concept,
        dcat:Resource ;
    rdfs:label "Item I986"@en-AU ;
    rdfs:comment "201 A  Person with knowledge of a computer or a computer system to assist access etc - GraphNodeID: I986"@en-AU ;
    skos:definition "201 A  Person with knowledge of a computer or a computer system to assist access etc"@en-AU ;
    skos:narrower C1901A00006:978 ;
    skos:prefLabel "Item I986"@en-AU ;
    dcat:accessURL "https://www.legislation.gov.au/C1901A00006/2024-07-01/2024-07-01/text/original/epub/OEBPS/document_3/document_3.html#_Toc172627020"^^xsd:anyURI .

C1901A00006:987 a legcons:Item,
        skos:Concept,
        dcat:Resource ;
    rdfs:label "Item I987"@en-AU ;
    rdfs:comment "201 B  Accessing data held on other premisesnotification to occupier of that premises - GraphNodeID: I987"@en-AU ;
    skos:definition "201 B  Accessing data held on other premisesnotification to occupier of that premises"@en-AU ;
    skos:narrower C1901A00006:978 ;
    skos:prefLabel "Item I987"@en-AU ;
    dcat:accessURL "https://www.legislation.gov.au/C1901A00006/2024-07-01/2024-07-01/text/original/epub/OEBPS/document_3/document_3.html#_Toc172627021"^^xsd:anyURI .

C1901A00006:988 a legcons:Item,
        skos:Concept,
        dcat:Resource ;
    rdfs:label "Item I988"@en-AU ;
    rdfs:comment "202  Compensation for damage to equipment or data - GraphNodeID: I988"@en-AU ;
    skos:definition "202  Compensation for damage to equipment or data"@en-AU ;
    skos:narrower C1901A00006:978 ;
    skos:prefLabel "Item I988"@en-AU ;
    dcat:accessURL "https://www.legislation.gov.au/C1901A00006/2024-07-01/2024-07-01/text/original/epub/OEBPS/document_3/document_3.html#_Toc172627022"^^xsd:anyURI .

C1901A00006:989 a legcons:Item,
        skos:Concept,
        dcat:Resource ;
    rdfs:label "Item I989"@en-AU ;
    rdfs:comment "202 A  Copies of seized things to be provided - GraphNodeID: I989"@en-AU ;
    skos:definition "202 A  Copies of seized things to be provided"@en-AU ;
    skos:narrower C1901A00006:978 ;
    skos:prefLabel "Item I989"@en-AU ;
    dcat:accessURL "https://www.legislation.gov.au/C1901A00006/2024-07-01/2024-07-01/text/original/epub/OEBPS/document_3/document_3.html#_Toc172627023"^^xsd:anyURI .

C1901A00006:990 a legcons:Item,
        skos:Concept,
        dcat:Resource ;
    rdfs:label "Item I990"@en-AU ;
    rdfs:comment "202 B  Relationship of this Subdivision to parliamentary privileges and immunities - GraphNodeID: I990"@en-AU ;
    skos:definition "202 B  Relationship of this Subdivision to parliamentary privileges and immunities"@en-AU ;
    skos:narrower C1901A00006:978 ;
    skos:prefLabel "Item I990"@en-AU ;
    dcat:accessURL "https://www.legislation.gov.au/C1901A00006/2024-07-01/2024-07-01/text/original/epub/OEBPS/document_3/document_3.html#_Toc172627024"^^xsd:anyURI .

C1901A00006:992 a legcons:Item,
        skos:Concept,
        dcat:Resource ;
    rdfs:label "Item I992"@en-AU ;
    rdfs:comment "203  When seizure warrants for forfeited goods can be issued - GraphNodeID: I992"@en-AU ;
    skos:definition "203  When seizure warrants for forfeited goods can be issued"@en-AU ;
    skos:narrower C1901A00006:991 ;
    skos:prefLabel "Item I992"@en-AU ;
    dcat:accessURL "https://www.legislation.gov.au/C1901A00006/2024-07-01/2024-07-01/text/original/epub/OEBPS/document_3/document_3.html#_Toc172627026"^^xsd:anyURI .

C1901A00006:993 a legcons:Item,
        skos:Concept,
        dcat:Resource ;
    rdfs:label "Item I993"@en-AU ;
    rdfs:comment "203 A  The things that are authorised by seizure warrants for forfeited goods - GraphNodeID: I993"@en-AU ;
    skos:definition "203 A  The things that are authorised by seizure warrants for forfeited goods"@en-AU ;
    skos:narrower C1901A00006:991 ;
    skos:prefLabel "Item I993"@en-AU ;
    dcat:accessURL "https://www.legislation.gov.au/C1901A00006/2024-07-01/2024-07-01/text/original/epub/OEBPS/document_3/document_3.html#_Toc172627027"^^xsd:anyURI .

C1901A00006:994 a legcons:Item,
        skos:Concept,
        dcat:Resource ;
    rdfs:label "Item I994"@en-AU ;
    rdfs:comment "203 B  Seizure without warrant of special forfeited goods or of evidential material relating to special forfeited goods at a Customs place - GraphNodeID: I994"@en-AU ;
    skos:definition "203 B  Seizure without warrant of special forfeited goods or of evidential material relating to special forfeited goods at a Customs place"@en-AU ;
    skos:narrower C1901A00006:991 ;
    skos:prefLabel "Item I994"@en-AU ;
    dcat:accessURL "https://www.legislation.gov.au/C1901A00006/2024-07-01/2024-07-01/text/original/epub/OEBPS/document_3/document_3.html#_Toc172627028"^^xsd:anyURI .

C1901A00006:995 a legcons:Item,
        skos:Concept,
        dcat:Resource ;
    rdfs:label "Item I995"@en-AU ;
    rdfs:comment "203 C  Seizure without warrant of narcotic goods or of evidential material relating to narcotic goods at other places - GraphNodeID: I995"@en-AU ;
    skos:definition "203 C  Seizure without warrant of narcotic goods or of evidential material relating to narcotic goods at other places"@en-AU ;
    skos:narrower C1901A00006:991 ;
    skos:prefLabel "Item I995"@en-AU ;
    dcat:accessURL "https://www.legislation.gov.au/C1901A00006/2024-07-01/2024-07-01/text/original/epub/OEBPS/document_3/document_3.html#_Toc172627029"^^xsd:anyURI .

C1901A00006:996 a legcons:Item,
        skos:Concept,
        dcat:Resource ;
    rdfs:label "Item I996"@en-AU ;
    rdfs:comment "203 CA  Seizure without warrant of certain goods on ship or aircraft in the Protected Zone - GraphNodeID: I996"@en-AU ;
    skos:definition "203 CA  Seizure without warrant of certain goods on ship or aircraft in the Protected Zone"@en-AU ;
    skos:narrower C1901A00006:991 ;
    skos:prefLabel "Item I996"@en-AU ;
    dcat:accessURL "https://www.legislation.gov.au/C1901A00006/2024-07-01/2024-07-01/text/original/epub/OEBPS/document_3/document_3.html#_Toc172627030"^^xsd:anyURI .

C1901A00006:997 a legcons:Item,
        skos:Concept,
        dcat:Resource ;
    rdfs:label "Item I997"@en-AU ;
    rdfs:comment "203 CB  Seizure without warrant of certain other goods in the Protected Zone - GraphNodeID: I997"@en-AU ;
    skos:definition "203 CB  Seizure without warrant of certain other goods in the Protected Zone"@en-AU ;
    skos:narrower C1901A00006:991 ;
    skos:prefLabel "Item I997"@en-AU ;
    dcat:accessURL "https://www.legislation.gov.au/C1901A00006/2024-07-01/2024-07-01/text/original/epub/OEBPS/document_3/document_3.html#_Toc172627031"^^xsd:anyURI .

C1901A00006:998 a legcons:Item,
        skos:Concept,
        dcat:Resource ;
    rdfs:label "Item I998"@en-AU ;
    rdfs:comment "203 D  How an authorised person is to exercise certain powers - GraphNodeID: I998"@en-AU ;
    skos:definition "203 D  How an authorised person is to exercise certain powers"@en-AU ;
    skos:narrower C1901A00006:991 ;
    skos:prefLabel "Item I998"@en-AU ;
    dcat:accessURL "https://www.legislation.gov.au/C1901A00006/2024-07-01/2024-07-01/text/original/epub/OEBPS/document_3/document_3.html#_Toc172627032"^^xsd:anyURI .

C1901A00006:1330 a legcons:Subdivision,
        skos:Concept,
        dcat:Resource ;
    rdfs:label "Subdivision S1330"@en-AU ;
    rdfs:comment "Subdivision APreliminary - GraphNodeID: S1330"@en-AU ;
    skos:broader C1901A00006:1331 ;
    skos:definition "Subdivision APreliminary"@en-AU ;
    skos:narrower C1901A00006:1329 ;
    skos:prefLabel "Subdivision S1330"@en-AU ;
    dcat:accessURL "https://www.legislation.gov.au/C1901A00006/2024-07-01/2024-07-01/text/original/epub/OEBPS/document_4/document_4.html#_Toc172628764"^^xsd:anyURI .

C1901A00006:1348 a legcons:Subdivision,
        skos:Concept,
        dcat:Resource ;
    rdfs:label "Subdivision S1348"@en-AU ;
    rdfs:comment "Subdivision DStaff assisting the Commissioner - GraphNodeID: S1348"@en-AU ;
    skos:broader C1901A00006:1349 ;
    skos:definition "Subdivision DStaff assisting the Commissioner"@en-AU ;
    skos:narrower C1901A00006:1329 ;
    skos:prefLabel "Subdivision S1348"@en-AU ;
    dcat:accessURL "https://www.legislation.gov.au/C1901A00006/2024-07-01/2024-07-01/text/original/epub/OEBPS/document_4/document_4.html#_Toc172628782"^^xsd:anyURI .

C1901A00006:1350 a legcons:Subdivision,
        skos:Concept,
        dcat:Resource ;
    rdfs:label "Subdivision S1350"@en-AU ;
    rdfs:comment "Subdivision EDelegation - GraphNodeID: S1350"@en-AU ;
    skos:broader C1901A00006:1351 ;
    skos:definition "Subdivision EDelegation"@en-AU ;
    skos:narrower C1901A00006:1329 ;
    skos:prefLabel "Subdivision S1350"@en-AU ;
    dcat:accessURL "https://www.legislation.gov.au/C1901A00006/2024-07-01/2024-07-01/text/original/epub/OEBPS/document_4/document_4.html#_Toc172628784"^^xsd:anyURI .

C1901A00006:1352 a legcons:Subdivision,
        skos:Concept,
        dcat:Resource ;
    rdfs:label "Subdivision S1352"@en-AU ;
    rdfs:comment "Subdivision FForm and manner of applications - GraphNodeID: S1352"@en-AU ;
    skos:broader C1901A00006:1353 ;
    skos:definition "Subdivision FForm and manner of applications"@en-AU ;
    skos:narrower C1901A00006:1329 ;
    skos:prefLabel "Subdivision S1352"@en-AU ;
    dcat:accessURL "https://www.legislation.gov.au/C1901A00006/2024-07-01/2024-07-01/text/original/epub/OEBPS/document_4/document_4.html#_Toc172628786"^^xsd:anyURI .

C1901A00006:524 a legcons:Subdivision,
        skos:Concept,
        dcat:Resource ;
    rdfs:label "Subdivision S524"@en-AU ;
    rdfs:comment "Subdivision BGoods wholly obtained or produced entirely in Singapore or in Singapore and Australia - GraphNodeID: S524"@en-AU ;
    skos:broader C1901A00006:525 ;
    skos:definition "Subdivision BGoods wholly obtained or produced entirely in Singapore or in Singapore and Australia"@en-AU ;
    skos:narrower C1901A00006:520 ;
    skos:prefLabel "Subdivision S524"@en-AU ;
    dcat:accessURL "https://www.legislation.gov.au/C1901A00006/2024-07-01/2024-07-01/text/original/epub/OEBPS/document_2/document_2.html#_Toc172624279"^^xsd:anyURI .

C1901A00006:526 a legcons:Subdivision,
        skos:Concept,
        dcat:Resource ;
    rdfs:label "Subdivision S526"@en-AU ;
    rdfs:comment "Subdivision CGoods produced in Singapore or in Singapore and Australia from originating materials - GraphNodeID: S526"@en-AU ;
    skos:broader C1901A00006:527 ;
    skos:definition "Subdivision CGoods produced in Singapore or in Singapore and Australia from originating materials"@en-AU ;
    skos:narrower C1901A00006:520 ;
    skos:prefLabel "Subdivision S526"@en-AU ;
    dcat:accessURL "https://www.legislation.gov.au/C1901A00006/2024-07-01/2024-07-01/text/original/epub/OEBPS/document_2/document_2.html#_Toc172624281"^^xsd:anyURI .

C1901A00006:531 a legcons:Subdivision,
        skos:Concept,
        dcat:Resource ;
    rdfs:label "Subdivision S531"@en-AU ;
    rdfs:comment "Subdivision EGoods that are accessories spare parts tools or instructional or other information materials - GraphNodeID: S531"@en-AU ;
    skos:broader C1901A00006:532 ;
    skos:definition "Subdivision EGoods that are accessories spare parts tools or instructional or other information materials"@en-AU ;
    skos:narrower C1901A00006:520 ;
    skos:prefLabel "Subdivision S531"@en-AU ;
    dcat:accessURL "https://www.legislation.gov.au/C1901A00006/2024-07-01/2024-07-01/text/original/epub/OEBPS/document_2/document_2.html#_Toc172624286"^^xsd:anyURI .

C1901A00006:533 a legcons:Subdivision,
        skos:Concept,
        dcat:Resource ;
    rdfs:label "Subdivision S533"@en-AU ;
    rdfs:comment "Subdivision FConsignment - GraphNodeID: S533"@en-AU ;
    skos:broader C1901A00006:534 ;
    skos:definition "Subdivision FConsignment"@en-AU ;
    skos:narrower C1901A00006:520 ;
    skos:prefLabel "Subdivision S533"@en-AU ;
    dcat:accessURL "https://www.legislation.gov.au/C1901A00006/2024-07-01/2024-07-01/text/original/epub/OEBPS/document_2/document_2.html#_Toc172624288"^^xsd:anyURI .

C1901A00006:535 a legcons:Subdivision,
        skos:Concept,
        dcat:Resource ;
    rdfs:label "Subdivision S535"@en-AU ;
    rdfs:comment "Subdivision GRegulations - GraphNodeID: S535"@en-AU ;
    skos:broader C1901A00006:536 ;
    skos:definition "Subdivision GRegulations"@en-AU ;
    skos:narrower C1901A00006:520 ;
    skos:prefLabel "Subdivision S535"@en-AU ;
    dcat:accessURL "https://www.legislation.gov.au/C1901A00006/2024-07-01/2024-07-01/text/original/epub/OEBPS/document_2/document_2.html#_Toc172624290"^^xsd:anyURI .

C1901A00006:541 a legcons:Subdivision,
        skos:Concept,
        dcat:Resource ;
    rdfs:label "Subdivision S541"@en-AU ;
    rdfs:comment "Subdivision BGoods wholly obtained or produced entirely in the US - GraphNodeID: S541"@en-AU ;
    skos:broader C1901A00006:542 ;
    skos:definition "Subdivision BGoods wholly obtained or produced entirely in the US"@en-AU ;
    skos:narrower C1901A00006:537 ;
    skos:prefLabel "Subdivision S541"@en-AU ;
    dcat:accessURL "https://www.legislation.gov.au/C1901A00006/2024-07-01/2024-07-01/text/original/epub/OEBPS/document_2/document_2.html#_Toc172624296"^^xsd:anyURI .

C1901A00006:543 a legcons:Subdivision,
        skos:Concept,
        dcat:Resource ;
    rdfs:label "Subdivision S543"@en-AU ;
    rdfs:comment "Subdivision CGoods produced entirely in the US or in the US and Australia exclusively from originating materials - GraphNodeID: S543"@en-AU ;
    skos:broader C1901A00006:544 ;
    skos:definition "Subdivision CGoods produced entirely in the US or in the US and Australia exclusively from originating materials"@en-AU ;
    skos:narrower C1901A00006:537 ;
    skos:prefLabel "Subdivision S543"@en-AU ;
    dcat:accessURL "https://www.legislation.gov.au/C1901A00006/2024-07-01/2024-07-01/text/original/epub/OEBPS/document_2/document_2.html#_Toc172624298"^^xsd:anyURI .

C1901A00006:545 a legcons:Subdivision,
        skos:Concept,
        dcat:Resource ;
    rdfs:label "Subdivision S545"@en-AU ;
    rdfs:comment "Subdivision DGoods produced in the US or in the US and Australia from non originating materials - GraphNodeID: S545"@en-AU ;
    skos:broader C1901A00006:546 ;
    skos:definition "Subdivision DGoods produced in the US or in the US and Australia from non originating materials"@en-AU ;
    skos:narrower C1901A00006:537 ;
    skos:prefLabel "Subdivision S545"@en-AU ;
    dcat:accessURL "https://www.legislation.gov.au/C1901A00006/2024-07-01/2024-07-01/text/original/epub/OEBPS/document_2/document_2.html#_Toc172624300"^^xsd:anyURI .

C1901A00006:547 a legcons:Subdivision,
        skos:Concept,
        dcat:Resource ;
    rdfs:label "Subdivision S547"@en-AU ;
    rdfs:comment "Subdivision FGoods that are standard accessories spare parts or tools - GraphNodeID: S547"@en-AU ;
    skos:broader C1901A00006:548 ;
    skos:definition "Subdivision FGoods that are standard accessories spare parts or tools"@en-AU ;
    skos:narrower C1901A00006:537 ;
    skos:prefLabel "Subdivision S547"@en-AU ;
    dcat:accessURL "https://www.legislation.gov.au/C1901A00006/2024-07-01/2024-07-01/text/original/epub/OEBPS/document_2/document_2.html#_Toc172624302"^^xsd:anyURI .

C1901A00006:549 a legcons:Subdivision,
        skos:Concept,
        dcat:Resource ;
    rdfs:label "Subdivision S549"@en-AU ;
    rdfs:comment "Subdivision GPackaging materials and containers - GraphNodeID: S549"@en-AU ;
    skos:broader C1901A00006:550 ;
    skos:definition "Subdivision GPackaging materials and containers"@en-AU ;
    skos:narrower C1901A00006:537 ;
    skos:prefLabel "Subdivision S549"@en-AU ;
    dcat:accessURL "https://www.legislation.gov.au/C1901A00006/2024-07-01/2024-07-01/text/original/epub/OEBPS/document_2/document_2.html#_Toc172624304"^^xsd:anyURI .

C1901A00006:551 a legcons:Subdivision,
        skos:Concept,
        dcat:Resource ;
    rdfs:label "Subdivision S551"@en-AU ;
    rdfs:comment "Subdivision HConsignment - GraphNodeID: S551"@en-AU ;
    skos:broader C1901A00006:552 ;
    skos:definition "Subdivision HConsignment"@en-AU ;
    skos:narrower C1901A00006:537 ;
    skos:prefLabel "Subdivision S551"@en-AU ;
    dcat:accessURL "https://www.legislation.gov.au/C1901A00006/2024-07-01/2024-07-01/text/original/epub/OEBPS/document_2/document_2.html#_Toc172624306"^^xsd:anyURI .

C1901A00006:553 a legcons:Subdivision,
        skos:Concept,
        dcat:Resource ;
    rdfs:label "Subdivision S553"@en-AU ;
    rdfs:comment "Subdivision IRegulations - GraphNodeID: S553"@en-AU ;
    skos:broader C1901A00006:554 ;
    skos:definition "Subdivision IRegulations"@en-AU ;
    skos:narrower C1901A00006:537 ;
    skos:prefLabel "Subdivision S553"@en-AU ;
    dcat:accessURL "https://www.legislation.gov.au/C1901A00006/2024-07-01/2024-07-01/text/original/epub/OEBPS/document_2/document_2.html#_Toc172624308"^^xsd:anyURI .

C1901A00006:559 a legcons:Subdivision,
        skos:Concept,
        dcat:Resource ;
    rdfs:label "Subdivision S559"@en-AU ;
    rdfs:comment "Subdivision BWholly obtained goods of Thailand - GraphNodeID: S559"@en-AU ;
    skos:broader C1901A00006:560 ;
    skos:definition "Subdivision BWholly obtained goods of Thailand"@en-AU ;
    skos:narrower C1901A00006:555 ;
    skos:prefLabel "Subdivision S559"@en-AU ;
    dcat:accessURL "https://www.legislation.gov.au/C1901A00006/2024-07-01/2024-07-01/text/original/epub/OEBPS/document_2/document_2.html#_Toc172624314"^^xsd:anyURI .

C1901A00006:561 a legcons:Subdivision,
        skos:Concept,
        dcat:Resource ;
    rdfs:label "Subdivision S561"@en-AU ;
    rdfs:comment "Subdivision CGoods produced entirely in Thailand or in Thailand and Australia - GraphNodeID: S561"@en-AU ;
    skos:broader C1901A00006:562 ;
    skos:definition "Subdivision CGoods produced entirely in Thailand or in Thailand and Australia"@en-AU ;
    skos:narrower C1901A00006:555 ;
    skos:prefLabel "Subdivision S561"@en-AU ;
    dcat:accessURL "https://www.legislation.gov.au/C1901A00006/2024-07-01/2024-07-01/text/original/epub/OEBPS/document_2/document_2.html#_Toc172624316"^^xsd:anyURI .

C1901A00006:563 a legcons:Subdivision,
        skos:Concept,
        dcat:Resource ;
    rdfs:label "Subdivision S563"@en-AU ;
    rdfs:comment "Subdivision DGoods that are standard accessories spare parts or tools - GraphNodeID: S563"@en-AU ;
    skos:broader C1901A00006:564 ;
    skos:definition "Subdivision DGoods that are standard accessories spare parts or tools"@en-AU ;
    skos:narrower C1901A00006:555 ;
    skos:prefLabel "Subdivision S563"@en-AU ;
    dcat:accessURL "https://www.legislation.gov.au/C1901A00006/2024-07-01/2024-07-01/text/original/epub/OEBPS/document_2/document_2.html#_Toc172624318"^^xsd:anyURI .

C1901A00006:565 a legcons:Subdivision,
        skos:Concept,
        dcat:Resource ;
    rdfs:label "Subdivision S565"@en-AU ;
    rdfs:comment "Subdivision EPackaging materials and containers - GraphNodeID: S565"@en-AU ;
    skos:broader C1901A00006:566 ;
    skos:definition "Subdivision EPackaging materials and containers"@en-AU ;
    skos:narrower C1901A00006:555 ;
    skos:prefLabel "Subdivision S565"@en-AU ;
    dcat:accessURL "https://www.legislation.gov.au/C1901A00006/2024-07-01/2024-07-01/text/original/epub/OEBPS/document_2/document_2.html#_Toc172624320"^^xsd:anyURI .

C1901A00006:567 a legcons:Subdivision,
        skos:Concept,
        dcat:Resource ;
    rdfs:label "Subdivision S567"@en-AU ;
    rdfs:comment "Subdivision FConsignment - GraphNodeID: S567"@en-AU ;
    skos:broader C1901A00006:568 ;
    skos:definition "Subdivision FConsignment"@en-AU ;
    skos:narrower C1901A00006:555 ;
    skos:prefLabel "Subdivision S567"@en-AU ;
    dcat:accessURL "https://www.legislation.gov.au/C1901A00006/2024-07-01/2024-07-01/text/original/epub/OEBPS/document_2/document_2.html#_Toc172624322"^^xsd:anyURI .

C1901A00006:569 a legcons:Subdivision,
        skos:Concept,
        dcat:Resource ;
    rdfs:label "Subdivision S569"@en-AU ;
    rdfs:comment "Subdivision GRegulations - GraphNodeID: S569"@en-AU ;
    skos:broader C1901A00006:570 ;
    skos:definition "Subdivision GRegulations"@en-AU ;
    skos:narrower C1901A00006:555 ;
    skos:prefLabel "Subdivision S569"@en-AU ;
    dcat:accessURL "https://www.legislation.gov.au/C1901A00006/2024-07-01/2024-07-01/text/original/epub/OEBPS/document_2/document_2.html#_Toc172624324"^^xsd:anyURI .

C1901A00006:575 a legcons:Subdivision,
        skos:Concept,
        dcat:Resource ;
    rdfs:label "Subdivision S575"@en-AU ;
    rdfs:comment "Subdivision BGoods wholly obtained or produced in New Zealand or New Zealand and Australia - GraphNodeID: S575"@en-AU ;
    skos:broader C1901A00006:576 ;
    skos:definition "Subdivision BGoods wholly obtained or produced in New Zealand or New Zealand and Australia"@en-AU ;
    skos:narrower C1901A00006:571 ;
    skos:prefLabel "Subdivision S575"@en-AU ;
    dcat:accessURL "https://www.legislation.gov.au/C1901A00006/2024-07-01/2024-07-01/text/original/epub/OEBPS/document_2/document_2.html#_Toc172624330"^^xsd:anyURI .

C1901A00006:577 a legcons:Subdivision,
        skos:Concept,
        dcat:Resource ;
    rdfs:label "Subdivision S577"@en-AU ;
    rdfs:comment "Subdivision CGoods produced in New Zealand or New Zealand and Australia from originating materials - GraphNodeID: S577"@en-AU ;
    skos:broader C1901A00006:578 ;
    skos:definition "Subdivision CGoods produced in New Zealand or New Zealand and Australia from originating materials"@en-AU ;
    skos:narrower C1901A00006:571 ;
    skos:prefLabel "Subdivision S577"@en-AU ;
    dcat:accessURL "https://www.legislation.gov.au/C1901A00006/2024-07-01/2024-07-01/text/original/epub/OEBPS/document_2/document_2.html#_Toc172624332"^^xsd:anyURI .

C1901A00006:582 a legcons:Subdivision,
        skos:Concept,
        dcat:Resource ;
    rdfs:label "Subdivision S582"@en-AU ;
    rdfs:comment "Subdivision EGoods that are standard accessories spare parts or tools - GraphNodeID: S582"@en-AU ;
    skos:broader C1901A00006:583 ;
    skos:definition "Subdivision EGoods that are standard accessories spare parts or tools"@en-AU ;
    skos:narrower C1901A00006:571 ;
    skos:prefLabel "Subdivision S582"@en-AU ;
    dcat:accessURL "https://www.legislation.gov.au/C1901A00006/2024-07-01/2024-07-01/text/original/epub/OEBPS/document_2/document_2.html#_Toc172624337"^^xsd:anyURI .

C1901A00006:584 a legcons:Subdivision,
        skos:Concept,
        dcat:Resource ;
    rdfs:label "Subdivision S584"@en-AU ;
    rdfs:comment "Subdivision FGoods wholly manufactured in New Zealand - GraphNodeID: S584"@en-AU ;
    skos:broader C1901A00006:585 ;
    skos:definition "Subdivision FGoods wholly manufactured in New Zealand"@en-AU ;
    skos:narrower C1901A00006:571 ;
    skos:prefLabel "Subdivision S584"@en-AU ;
    dcat:accessURL "https://www.legislation.gov.au/C1901A00006/2024-07-01/2024-07-01/text/original/epub/OEBPS/document_2/document_2.html#_Toc172624339"^^xsd:anyURI .

C1901A00006:586 a legcons:Subdivision,
        skos:Concept,
        dcat:Resource ;
    rdfs:label "Subdivision S586"@en-AU ;
    rdfs:comment "Subdivision GNon qualifying operations - GraphNodeID: S586"@en-AU ;
    skos:broader C1901A00006:587 ;
    skos:definition "Subdivision GNon qualifying operations"@en-AU ;
    skos:narrower C1901A00006:571 ;
    skos:prefLabel "Subdivision S586"@en-AU ;
    dcat:accessURL "https://www.legislation.gov.au/C1901A00006/2024-07-01/2024-07-01/text/original/epub/OEBPS/document_2/document_2.html#_Toc172624341"^^xsd:anyURI .

C1901A00006:588 a legcons:Subdivision,
        skos:Concept,
        dcat:Resource ;
    rdfs:label "Subdivision S588"@en-AU ;
    rdfs:comment "Subdivision HConsignment - GraphNodeID: S588"@en-AU ;
    skos:broader C1901A00006:589 ;
    skos:definition "Subdivision HConsignment"@en-AU ;
    skos:narrower C1901A00006:571 ;
    skos:prefLabel "Subdivision S588"@en-AU ;
    dcat:accessURL "https://www.legislation.gov.au/C1901A00006/2024-07-01/2024-07-01/text/original/epub/OEBPS/document_2/document_2.html#_Toc172624343"^^xsd:anyURI .

C1901A00006:590 a legcons:Subdivision,
        skos:Concept,
        dcat:Resource ;
    rdfs:label "Subdivision S590"@en-AU ;
    rdfs:comment "Subdivision IRegulations - GraphNodeID: S590"@en-AU ;
    skos:broader C1901A00006:591 ;
    skos:definition "Subdivision IRegulations"@en-AU ;
    skos:narrower C1901A00006:571 ;
    skos:prefLabel "Subdivision S590"@en-AU ;
    dcat:accessURL "https://www.legislation.gov.au/C1901A00006/2024-07-01/2024-07-01/text/original/epub/OEBPS/document_2/document_2.html#_Toc172624345"^^xsd:anyURI .

C1901A00006:596 a legcons:Subdivision,
        skos:Concept,
        dcat:Resource ;
    rdfs:label "Subdivision S596"@en-AU ;
    rdfs:comment "Subdivision BGoods wholly obtained or produced entirely in Peru or in Peru and Australia - GraphNodeID: S596"@en-AU ;
    skos:broader C1901A00006:597 ;
    skos:definition "Subdivision BGoods wholly obtained or produced entirely in Peru or in Peru and Australia"@en-AU ;
    skos:narrower C1901A00006:592 ;
    skos:prefLabel "Subdivision S596"@en-AU ;
    dcat:accessURL "https://www.legislation.gov.au/C1901A00006/2024-07-01/2024-07-01/text/original/epub/OEBPS/document_2/document_2.html#_Toc172624351"^^xsd:anyURI .

C1901A00006:598 a legcons:Subdivision,
        skos:Concept,
        dcat:Resource ;
    rdfs:label "Subdivision S598"@en-AU ;
    rdfs:comment "Subdivision CGoods produced in Peru or in Peru and Australia from originating materials - GraphNodeID: S598"@en-AU ;
    skos:broader C1901A00006:599 ;
    skos:definition "Subdivision CGoods produced in Peru or in Peru and Australia from originating materials"@en-AU ;
    skos:narrower C1901A00006:592 ;
    skos:prefLabel "Subdivision S598"@en-AU ;
    dcat:accessURL "https://www.legislation.gov.au/C1901A00006/2024-07-01/2024-07-01/text/original/epub/OEBPS/document_2/document_2.html#_Toc172624353"^^xsd:anyURI .

C1901A00006:603 a legcons:Subdivision,
        skos:Concept,
        dcat:Resource ;
    rdfs:label "Subdivision S603"@en-AU ;
    rdfs:comment "Subdivision EGoods that are accessories spare parts tools or instructional or other information materials - GraphNodeID: S603"@en-AU ;
    skos:broader C1901A00006:604 ;
    skos:definition "Subdivision EGoods that are accessories spare parts tools or instructional or other information materials"@en-AU ;
    skos:narrower C1901A00006:592 ;
    skos:prefLabel "Subdivision S603"@en-AU ;
    dcat:accessURL "https://www.legislation.gov.au/C1901A00006/2024-07-01/2024-07-01/text/original/epub/OEBPS/document_2/document_2.html#_Toc172624358"^^xsd:anyURI .

C1901A00006:605 a legcons:Subdivision,
        skos:Concept,
        dcat:Resource ;
    rdfs:label "Subdivision S605"@en-AU ;
    rdfs:comment "Subdivision FConsignment - GraphNodeID: S605"@en-AU ;
    skos:broader C1901A00006:606 ;
    skos:definition "Subdivision FConsignment"@en-AU ;
    skos:narrower C1901A00006:592 ;
    skos:prefLabel "Subdivision S605"@en-AU ;
    dcat:accessURL "https://www.legislation.gov.au/C1901A00006/2024-07-01/2024-07-01/text/original/epub/OEBPS/document_2/document_2.html#_Toc172624360"^^xsd:anyURI .

C1901A00006:607 a legcons:Subdivision,
        skos:Concept,
        dcat:Resource ;
    rdfs:label "Subdivision S607"@en-AU ;
    rdfs:comment "Subdivision GRegulations - GraphNodeID: S607"@en-AU ;
    skos:broader C1901A00006:608 ;
    skos:definition "Subdivision GRegulations"@en-AU ;
    skos:narrower C1901A00006:592 ;
    skos:prefLabel "Subdivision S607"@en-AU ;
    dcat:accessURL "https://www.legislation.gov.au/C1901A00006/2024-07-01/2024-07-01/text/original/epub/OEBPS/document_2/document_2.html#_Toc172624362"^^xsd:anyURI .

C1901A00006:613 a legcons:Subdivision,
        skos:Concept,
        dcat:Resource ;
    rdfs:label "Subdivision S613"@en-AU ;
    rdfs:comment "Subdivision BWholly obtained goods of Chile - GraphNodeID: S613"@en-AU ;
    skos:broader C1901A00006:614 ;
    skos:definition "Subdivision BWholly obtained goods of Chile"@en-AU ;
    skos:narrower C1901A00006:609 ;
    skos:prefLabel "Subdivision S613"@en-AU ;
    dcat:accessURL "https://www.legislation.gov.au/C1901A00006/2024-07-01/2024-07-01/text/original/epub/OEBPS/document_2/document_2.html#_Toc172624368"^^xsd:anyURI .

C1901A00006:615 a legcons:Subdivision,
        skos:Concept,
        dcat:Resource ;
    rdfs:label "Subdivision S615"@en-AU ;
    rdfs:comment "Subdivision CGoods produced in Chile from originating materials - GraphNodeID: S615"@en-AU ;
    skos:broader C1901A00006:616 ;
    skos:definition "Subdivision CGoods produced in Chile from originating materials"@en-AU ;
    skos:narrower C1901A00006:609 ;
    skos:prefLabel "Subdivision S615"@en-AU ;
    dcat:accessURL "https://www.legislation.gov.au/C1901A00006/2024-07-01/2024-07-01/text/original/epub/OEBPS/document_2/document_2.html#_Toc172624370"^^xsd:anyURI .

C1901A00006:620 a legcons:Subdivision,
        skos:Concept,
        dcat:Resource ;
    rdfs:label "Subdivision S620"@en-AU ;
    rdfs:comment "Subdivision EGoods that are accessories spare parts tools or instructional or other information resources - GraphNodeID: S620"@en-AU ;
    skos:broader C1901A00006:621 ;
    skos:definition "Subdivision EGoods that are accessories spare parts tools or instructional or other information resources"@en-AU ;
    skos:narrower C1901A00006:609 ;
    skos:prefLabel "Subdivision S620"@en-AU ;
    dcat:accessURL "https://www.legislation.gov.au/C1901A00006/2024-07-01/2024-07-01/text/original/epub/OEBPS/document_2/document_2.html#_Toc172624375"^^xsd:anyURI .

C1901A00006:622 a legcons:Subdivision,
        skos:Concept,
        dcat:Resource ;
    rdfs:label "Subdivision S622"@en-AU ;
    rdfs:comment "Subdivision FNon qualifying operations - GraphNodeID: S622"@en-AU ;
    skos:broader C1901A00006:623 ;
    skos:definition "Subdivision FNon qualifying operations"@en-AU ;
    skos:narrower C1901A00006:609 ;
    skos:prefLabel "Subdivision S622"@en-AU ;
    dcat:accessURL "https://www.legislation.gov.au/C1901A00006/2024-07-01/2024-07-01/text/original/epub/OEBPS/document_2/document_2.html#_Toc172624377"^^xsd:anyURI .

C1901A00006:624 a legcons:Subdivision,
        skos:Concept,
        dcat:Resource ;
    rdfs:label "Subdivision S624"@en-AU ;
    rdfs:comment "Subdivision GConsignment - GraphNodeID: S624"@en-AU ;
    skos:broader C1901A00006:625 ;
    skos:definition "Subdivision GConsignment"@en-AU ;
    skos:narrower C1901A00006:609 ;
    skos:prefLabel "Subdivision S624"@en-AU ;
    dcat:accessURL "https://www.legislation.gov.au/C1901A00006/2024-07-01/2024-07-01/text/original/epub/OEBPS/document_2/document_2.html#_Toc172624379"^^xsd:anyURI .

C1901A00006:626 a legcons:Subdivision,
        skos:Concept,
        dcat:Resource ;
    rdfs:label "Subdivision S626"@en-AU ;
    rdfs:comment "Subdivision HRegulations - GraphNodeID: S626"@en-AU ;
    skos:broader C1901A00006:627 ;
    skos:definition "Subdivision HRegulations"@en-AU ;
    skos:narrower C1901A00006:609 ;
    skos:prefLabel "Subdivision S626"@en-AU ;
    dcat:accessURL "https://www.legislation.gov.au/C1901A00006/2024-07-01/2024-07-01/text/original/epub/OEBPS/document_2/document_2.html#_Toc172624381"^^xsd:anyURI .

C1901A00006:632 a legcons:Subdivision,
        skos:Concept,
        dcat:Resource ;
    rdfs:label "Subdivision S632"@en-AU ;
    rdfs:comment "Subdivision BWholly obtained goods of a Party - GraphNodeID: S632"@en-AU ;
    skos:broader C1901A00006:633 ;
    skos:definition "Subdivision BWholly obtained goods of a Party"@en-AU ;
    skos:narrower C1901A00006:628 ;
    skos:prefLabel "Subdivision S632"@en-AU ;
    dcat:accessURL "https://www.legislation.gov.au/C1901A00006/2024-07-01/2024-07-01/text/original/epub/OEBPS/document_2/document_2.html#_Toc172624387"^^xsd:anyURI .

C1901A00006:634 a legcons:Subdivision,
        skos:Concept,
        dcat:Resource ;
    rdfs:label "Subdivision S634"@en-AU ;
    rdfs:comment "Subdivision CGoods produced from originating materials - GraphNodeID: S634"@en-AU ;
    skos:broader C1901A00006:635 ;
    skos:definition "Subdivision CGoods produced from originating materials"@en-AU ;
    skos:narrower C1901A00006:628 ;
    skos:prefLabel "Subdivision S634"@en-AU ;
    dcat:accessURL "https://www.legislation.gov.au/C1901A00006/2024-07-01/2024-07-01/text/original/epub/OEBPS/document_2/document_2.html#_Toc172624389"^^xsd:anyURI .

C1901A00006:640 a legcons:Subdivision,
        skos:Concept,
        dcat:Resource ;
    rdfs:label "Subdivision S640"@en-AU ;
    rdfs:comment "Subdivision EGoods that are accessories spare parts tools or instructional or other information materials - GraphNodeID: S640"@en-AU ;
    skos:broader C1901A00006:641 ;
    skos:definition "Subdivision EGoods that are accessories spare parts tools or instructional or other information materials"@en-AU ;
    skos:narrower C1901A00006:628 ;
    skos:prefLabel "Subdivision S640"@en-AU ;
    dcat:accessURL "https://www.legislation.gov.au/C1901A00006/2024-07-01/2024-07-01/text/original/epub/OEBPS/document_2/document_2.html#_Toc172624395"^^xsd:anyURI .

C1901A00006:642 a legcons:Subdivision,
        skos:Concept,
        dcat:Resource ;
    rdfs:label "Subdivision S642"@en-AU ;
    rdfs:comment "Subdivision FConsignment - GraphNodeID: S642"@en-AU ;
    skos:broader C1901A00006:643 ;
    skos:definition "Subdivision FConsignment"@en-AU ;
    skos:narrower C1901A00006:628 ;
    skos:prefLabel "Subdivision S642"@en-AU ;
    dcat:accessURL "https://www.legislation.gov.au/C1901A00006/2024-07-01/2024-07-01/text/original/epub/OEBPS/document_2/document_2.html#_Toc172624397"^^xsd:anyURI .

C1901A00006:644 a legcons:Subdivision,
        skos:Concept,
        dcat:Resource ;
    rdfs:label "Subdivision S644"@en-AU ;
    rdfs:comment "Subdivision GRegulations - GraphNodeID: S644"@en-AU ;
    skos:broader C1901A00006:645 ;
    skos:definition "Subdivision GRegulations"@en-AU ;
    skos:narrower C1901A00006:628 ;
    skos:prefLabel "Subdivision S644"@en-AU ;
    dcat:accessURL "https://www.legislation.gov.au/C1901A00006/2024-07-01/2024-07-01/text/original/epub/OEBPS/document_2/document_2.html#_Toc172624399"^^xsd:anyURI .

C1901A00006:650 a legcons:Subdivision,
        skos:Concept,
        dcat:Resource ;
    rdfs:label "Subdivision S650"@en-AU ;
    rdfs:comment "Subdivision BGoods wholly obtained or produced in a Party - GraphNodeID: S650"@en-AU ;
    skos:broader C1901A00006:651 ;
    skos:definition "Subdivision BGoods wholly obtained or produced in a Party"@en-AU ;
    skos:narrower C1901A00006:646 ;
    skos:prefLabel "Subdivision S650"@en-AU ;
    dcat:accessURL "https://www.legislation.gov.au/C1901A00006/2024-07-01/2024-07-01/text/original/epub/OEBPS/document_2/document_2.html#_Toc172624405"^^xsd:anyURI .

C1901A00006:652 a legcons:Subdivision,
        skos:Concept,
        dcat:Resource ;
    rdfs:label "Subdivision S652"@en-AU ;
    rdfs:comment "Subdivision CGoods produced from originating materials - GraphNodeID: S652"@en-AU ;
    skos:broader C1901A00006:653 ;
    skos:definition "Subdivision CGoods produced from originating materials"@en-AU ;
    skos:narrower C1901A00006:646 ;
    skos:prefLabel "Subdivision S652"@en-AU ;
    dcat:accessURL "https://www.legislation.gov.au/C1901A00006/2024-07-01/2024-07-01/text/original/epub/OEBPS/document_2/document_2.html#_Toc172624407"^^xsd:anyURI .

C1901A00006:657 a legcons:Subdivision,
        skos:Concept,
        dcat:Resource ;
    rdfs:label "Subdivision S657"@en-AU ;
    rdfs:comment "Subdivision EGoods that are accessories spare parts tools or instructional or other information materials - GraphNodeID: S657"@en-AU ;
    skos:broader C1901A00006:658 ;
    skos:definition "Subdivision EGoods that are accessories spare parts tools or instructional or other information materials"@en-AU ;
    skos:narrower C1901A00006:646 ;
    skos:prefLabel "Subdivision S657"@en-AU ;
    dcat:accessURL "https://www.legislation.gov.au/C1901A00006/2024-07-01/2024-07-01/text/original/epub/OEBPS/document_2/document_2.html#_Toc172624412"^^xsd:anyURI .

C1901A00006:659 a legcons:Subdivision,
        skos:Concept,
        dcat:Resource ;
    rdfs:label "Subdivision S659"@en-AU ;
    rdfs:comment "Subdivision FConsignment - GraphNodeID: S659"@en-AU ;
    skos:broader C1901A00006:660 ;
    skos:definition "Subdivision FConsignment"@en-AU ;
    skos:narrower C1901A00006:646 ;
    skos:prefLabel "Subdivision S659"@en-AU ;
    dcat:accessURL "https://www.legislation.gov.au/C1901A00006/2024-07-01/2024-07-01/text/original/epub/OEBPS/document_2/document_2.html#_Toc172624414"^^xsd:anyURI .

C1901A00006:661 a legcons:Subdivision,
        skos:Concept,
        dcat:Resource ;
    rdfs:label "Subdivision S661"@en-AU ;
    rdfs:comment "Subdivision GRegulations - GraphNodeID: S661"@en-AU ;
    skos:broader C1901A00006:662 ;
    skos:definition "Subdivision GRegulations"@en-AU ;
    skos:narrower C1901A00006:646 ;
    skos:prefLabel "Subdivision S661"@en-AU ;
    dcat:accessURL "https://www.legislation.gov.au/C1901A00006/2024-07-01/2024-07-01/text/original/epub/OEBPS/document_2/document_2.html#_Toc172624416"^^xsd:anyURI .

C1901A00006:667 a legcons:Subdivision,
        skos:Concept,
        dcat:Resource ;
    rdfs:label "Subdivision S667"@en-AU ;
    rdfs:comment "Subdivision BGoods wholly obtained or produced entirely in the territory of one or more of the Parties - GraphNodeID: S667"@en-AU ;
    skos:broader C1901A00006:668 ;
    skos:definition "Subdivision BGoods wholly obtained or produced entirely in the territory of one or more of the Parties"@en-AU ;
    skos:narrower C1901A00006:663 ;
    skos:prefLabel "Subdivision S667"@en-AU ;
    dcat:accessURL "https://www.legislation.gov.au/C1901A00006/2024-07-01/2024-07-01/text/original/epub/OEBPS/document_2/document_2.html#_Toc172624422"^^xsd:anyURI .

C1901A00006:669 a legcons:Subdivision,
        skos:Concept,
        dcat:Resource ;
    rdfs:label "Subdivision S669"@en-AU ;
    rdfs:comment "Subdivision CGoods produced from originating materials - GraphNodeID: S669"@en-AU ;
    skos:broader C1901A00006:670 ;
    skos:definition "Subdivision CGoods produced from originating materials"@en-AU ;
    skos:narrower C1901A00006:663 ;
    skos:prefLabel "Subdivision S669"@en-AU ;
    dcat:accessURL "https://www.legislation.gov.au/C1901A00006/2024-07-01/2024-07-01/text/original/epub/OEBPS/document_2/document_2.html#_Toc172624424"^^xsd:anyURI .

C1901A00006:674 a legcons:Subdivision,
        skos:Concept,
        dcat:Resource ;
    rdfs:label "Subdivision S674"@en-AU ;
    rdfs:comment "Subdivision EGoods that are accessories spare parts tools or instructional or other information materials - GraphNodeID: S674"@en-AU ;
    skos:broader C1901A00006:675 ;
    skos:definition "Subdivision EGoods that are accessories spare parts tools or instructional or other information materials"@en-AU ;
    skos:narrower C1901A00006:663 ;
    skos:prefLabel "Subdivision S674"@en-AU ;
    dcat:accessURL "https://www.legislation.gov.au/C1901A00006/2024-07-01/2024-07-01/text/original/epub/OEBPS/document_2/document_2.html#_Toc172624429"^^xsd:anyURI .

C1901A00006:676 a legcons:Subdivision,
        skos:Concept,
        dcat:Resource ;
    rdfs:label "Subdivision S676"@en-AU ;
    rdfs:comment "Subdivision FConsignment - GraphNodeID: S676"@en-AU ;
    skos:broader C1901A00006:677 ;
    skos:definition "Subdivision FConsignment"@en-AU ;
    skos:narrower C1901A00006:663 ;
    skos:prefLabel "Subdivision S676"@en-AU ;
    dcat:accessURL "https://www.legislation.gov.au/C1901A00006/2024-07-01/2024-07-01/text/original/epub/OEBPS/document_2/document_2.html#_Toc172624431"^^xsd:anyURI .

C1901A00006:678 a legcons:Subdivision,
        skos:Concept,
        dcat:Resource ;
    rdfs:label "Subdivision S678"@en-AU ;
    rdfs:comment "Subdivision GRegulations - GraphNodeID: S678"@en-AU ;
    skos:broader C1901A00006:679 ;
    skos:definition "Subdivision GRegulations"@en-AU ;
    skos:narrower C1901A00006:663 ;
    skos:prefLabel "Subdivision S678"@en-AU ;
    dcat:accessURL "https://www.legislation.gov.au/C1901A00006/2024-07-01/2024-07-01/text/original/epub/OEBPS/document_2/document_2.html#_Toc172624433"^^xsd:anyURI .

C1901A00006:684 a legcons:Subdivision,
        skos:Concept,
        dcat:Resource ;
    rdfs:label "Subdivision S684"@en-AU ;
    rdfs:comment "Subdivision BGoods wholly obtained or produced in Malaysia or in Malaysia and Australia - GraphNodeID: S684"@en-AU ;
    skos:broader C1901A00006:685 ;
    skos:definition "Subdivision BGoods wholly obtained or produced in Malaysia or in Malaysia and Australia"@en-AU ;
    skos:narrower C1901A00006:680 ;
    skos:prefLabel "Subdivision S684"@en-AU ;
    dcat:accessURL "https://www.legislation.gov.au/C1901A00006/2024-07-01/2024-07-01/text/original/epub/OEBPS/document_2/document_2.html#_Toc172624439"^^xsd:anyURI .

C1901A00006:686 a legcons:Subdivision,
        skos:Concept,
        dcat:Resource ;
    rdfs:label "Subdivision S686"@en-AU ;
    rdfs:comment "Subdivision CGoods produced in Malaysia or in Malaysia and Australia from originating materials - GraphNodeID: S686"@en-AU ;
    skos:broader C1901A00006:687 ;
    skos:definition "Subdivision CGoods produced in Malaysia or in Malaysia and Australia from originating materials"@en-AU ;
    skos:narrower C1901A00006:680 ;
    skos:prefLabel "Subdivision S686"@en-AU ;
    dcat:accessURL "https://www.legislation.gov.au/C1901A00006/2024-07-01/2024-07-01/text/original/epub/OEBPS/document_2/document_2.html#_Toc172624441"^^xsd:anyURI .

C1901A00006:692 a legcons:Subdivision,
        skos:Concept,
        dcat:Resource ;
    rdfs:label "Subdivision S692"@en-AU ;
    rdfs:comment "Subdivision EGoods that are accessories spare parts tools or instructional or other information materials - GraphNodeID: S692"@en-AU ;
    skos:broader C1901A00006:693 ;
    skos:definition "Subdivision EGoods that are accessories spare parts tools or instructional or other information materials"@en-AU ;
    skos:narrower C1901A00006:680 ;
    skos:prefLabel "Subdivision S692"@en-AU ;
    dcat:accessURL "https://www.legislation.gov.au/C1901A00006/2024-07-01/2024-07-01/text/original/epub/OEBPS/document_2/document_2.html#_Toc172624447"^^xsd:anyURI .

C1901A00006:694 a legcons:Subdivision,
        skos:Concept,
        dcat:Resource ;
    rdfs:label "Subdivision S694"@en-AU ;
    rdfs:comment "Subdivision FConsignment - GraphNodeID: S694"@en-AU ;
    skos:broader C1901A00006:695 ;
    skos:definition "Subdivision FConsignment"@en-AU ;
    skos:narrower C1901A00006:680 ;
    skos:prefLabel "Subdivision S694"@en-AU ;
    dcat:accessURL "https://www.legislation.gov.au/C1901A00006/2024-07-01/2024-07-01/text/original/epub/OEBPS/document_2/document_2.html#_Toc172624449"^^xsd:anyURI .

C1901A00006:696 a legcons:Subdivision,
        skos:Concept,
        dcat:Resource ;
    rdfs:label "Subdivision S696"@en-AU ;
    rdfs:comment "Subdivision GRegulations - GraphNodeID: S696"@en-AU ;
    skos:broader C1901A00006:697 ;
    skos:definition "Subdivision GRegulations"@en-AU ;
    skos:narrower C1901A00006:680 ;
    skos:prefLabel "Subdivision S696"@en-AU ;
    dcat:accessURL "https://www.legislation.gov.au/C1901A00006/2024-07-01/2024-07-01/text/original/epub/OEBPS/document_2/document_2.html#_Toc172624451"^^xsd:anyURI .

C1901A00006:702 a legcons:Subdivision,
        skos:Concept,
        dcat:Resource ;
    rdfs:label "Subdivision S702"@en-AU ;
    rdfs:comment "Subdivision BGoods wholly obtained or produced in Indonesia - GraphNodeID: S702"@en-AU ;
    skos:broader C1901A00006:703 ;
    skos:definition "Subdivision BGoods wholly obtained or produced in Indonesia"@en-AU ;
    skos:narrower C1901A00006:698 ;
    skos:prefLabel "Subdivision S702"@en-AU ;
    dcat:accessURL "https://www.legislation.gov.au/C1901A00006/2024-07-01/2024-07-01/text/original/epub/OEBPS/document_2/document_2.html#_Toc172624457"^^xsd:anyURI .

C1901A00006:704 a legcons:Subdivision,
        skos:Concept,
        dcat:Resource ;
    rdfs:label "Subdivision S704"@en-AU ;
    rdfs:comment "Subdivision CGoods produced in Indonesia from originating materials - GraphNodeID: S704"@en-AU ;
    skos:broader C1901A00006:705 ;
    skos:definition "Subdivision CGoods produced in Indonesia from originating materials"@en-AU ;
    skos:narrower C1901A00006:698 ;
    skos:prefLabel "Subdivision S704"@en-AU ;
    dcat:accessURL "https://www.legislation.gov.au/C1901A00006/2024-07-01/2024-07-01/text/original/epub/OEBPS/document_2/document_2.html#_Toc172624459"^^xsd:anyURI .

C1901A00006:712 a legcons:Subdivision,
        skos:Concept,
        dcat:Resource ;
    rdfs:label "Subdivision S712"@en-AU ;
    rdfs:comment "Subdivision FRegulations - GraphNodeID: S712"@en-AU ;
    skos:broader C1901A00006:713 ;
    skos:definition "Subdivision FRegulations"@en-AU ;
    skos:narrower C1901A00006:698 ;
    skos:prefLabel "Subdivision S712"@en-AU ;
    dcat:accessURL "https://www.legislation.gov.au/C1901A00006/2024-07-01/2024-07-01/text/original/epub/OEBPS/document_2/document_2.html#_Toc172624467"^^xsd:anyURI .

C1901A00006:718 a legcons:Subdivision,
        skos:Concept,
        dcat:Resource ;
    rdfs:label "Subdivision S718"@en-AU ;
    rdfs:comment "Subdivision BGoods wholly obtained in Korea or in Korea and Australia - GraphNodeID: S718"@en-AU ;
    skos:broader C1901A00006:719 ;
    skos:definition "Subdivision BGoods wholly obtained in Korea or in Korea and Australia"@en-AU ;
    skos:narrower C1901A00006:714 ;
    skos:prefLabel "Subdivision S718"@en-AU ;
    dcat:accessURL "https://www.legislation.gov.au/C1901A00006/2024-07-01/2024-07-01/text/original/epub/OEBPS/document_2/document_2.html#_Toc172624473"^^xsd:anyURI .

C1901A00006:720 a legcons:Subdivision,
        skos:Concept,
        dcat:Resource ;
    rdfs:label "Subdivision S720"@en-AU ;
    rdfs:comment "Subdivision CGoods produced in Korea or in Korea and Australia from originating materials - GraphNodeID: S720"@en-AU ;
    skos:broader C1901A00006:721 ;
    skos:definition "Subdivision CGoods produced in Korea or in Korea and Australia from originating materials"@en-AU ;
    skos:narrower C1901A00006:714 ;
    skos:prefLabel "Subdivision S720"@en-AU ;
    dcat:accessURL "https://www.legislation.gov.au/C1901A00006/2024-07-01/2024-07-01/text/original/epub/OEBPS/document_2/document_2.html#_Toc172624475"^^xsd:anyURI .

C1901A00006:725 a legcons:Subdivision,
        skos:Concept,
        dcat:Resource ;
    rdfs:label "Subdivision S725"@en-AU ;
    rdfs:comment "Subdivision ENon qualifying operations - GraphNodeID: S725"@en-AU ;
    skos:broader C1901A00006:726 ;
    skos:definition "Subdivision ENon qualifying operations"@en-AU ;
    skos:narrower C1901A00006:714 ;
    skos:prefLabel "Subdivision S725"@en-AU ;
    dcat:accessURL "https://www.legislation.gov.au/C1901A00006/2024-07-01/2024-07-01/text/original/epub/OEBPS/document_2/document_2.html#_Toc172624480"^^xsd:anyURI .

C1901A00006:735 a legcons:Subdivision,
        skos:Concept,
        dcat:Resource ;
    rdfs:label "Subdivision S735"@en-AU ;
    rdfs:comment "Subdivision BGoods wholly obtained or produced in India or in India and Australia - GraphNodeID: S735"@en-AU ;
    skos:broader C1901A00006:736 ;
    skos:definition "Subdivision BGoods wholly obtained or produced in India or in India and Australia"@en-AU ;
    skos:narrower C1901A00006:731 ;
    skos:prefLabel "Subdivision S735"@en-AU ;
    dcat:accessURL "https://www.legislation.gov.au/C1901A00006/2024-07-01/2024-07-01/text/original/epub/OEBPS/document_2/document_2.html#_Toc172624490"^^xsd:anyURI .

C1901A00006:740 a legcons:Subdivision,
        skos:Concept,
        dcat:Resource ;
    rdfs:label "Subdivision S740"@en-AU ;
    rdfs:comment "Subdivision DPackaging materials and containers - GraphNodeID: S740"@en-AU ;
    skos:broader C1901A00006:741 ;
    skos:definition "Subdivision DPackaging materials and containers"@en-AU ;
    skos:narrower C1901A00006:731 ;
    skos:prefLabel "Subdivision S740"@en-AU ;
    dcat:accessURL "https://www.legislation.gov.au/C1901A00006/2024-07-01/2024-07-01/text/original/epub/OEBPS/document_2/document_2.html#_Toc172624495"^^xsd:anyURI .

C1901A00006:742 a legcons:Subdivision,
        skos:Concept,
        dcat:Resource ;
    rdfs:label "Subdivision S742"@en-AU ;
    rdfs:comment "Subdivision EConsignment - GraphNodeID: S742"@en-AU ;
    skos:broader C1901A00006:743 ;
    skos:definition "Subdivision EConsignment"@en-AU ;
    skos:narrower C1901A00006:731 ;
    skos:prefLabel "Subdivision S742"@en-AU ;
    dcat:accessURL "https://www.legislation.gov.au/C1901A00006/2024-07-01/2024-07-01/text/original/epub/OEBPS/document_2/document_2.html#_Toc172624497"^^xsd:anyURI .

C1901A00006:744 a legcons:Subdivision,
        skos:Concept,
        dcat:Resource ;
    rdfs:label "Subdivision S744"@en-AU ;
    rdfs:comment "Subdivision FRegulations - GraphNodeID: S744"@en-AU ;
    skos:broader C1901A00006:745 ;
    skos:definition "Subdivision FRegulations"@en-AU ;
    skos:narrower C1901A00006:731 ;
    skos:prefLabel "Subdivision S744"@en-AU ;
    dcat:accessURL "https://www.legislation.gov.au/C1901A00006/2024-07-01/2024-07-01/text/original/epub/OEBPS/document_2/document_2.html#_Toc172624499"^^xsd:anyURI .

C1901A00006:750 a legcons:Subdivision,
        skos:Concept,
        dcat:Resource ;
    rdfs:label "Subdivision S750"@en-AU ;
    rdfs:comment "Subdivision BGoods wholly obtained in Japan - GraphNodeID: S750"@en-AU ;
    skos:broader C1901A00006:751 ;
    skos:definition "Subdivision BGoods wholly obtained in Japan"@en-AU ;
    skos:narrower C1901A00006:746 ;
    skos:prefLabel "Subdivision S750"@en-AU ;
    dcat:accessURL "https://www.legislation.gov.au/C1901A00006/2024-07-01/2024-07-01/text/original/epub/OEBPS/document_2/document_2.html#_Toc172624505"^^xsd:anyURI .

C1901A00006:752 a legcons:Subdivision,
        skos:Concept,
        dcat:Resource ;
    rdfs:label "Subdivision S752"@en-AU ;
    rdfs:comment "Subdivision CGoods produced in Japan from originating materials - GraphNodeID: S752"@en-AU ;
    skos:broader C1901A00006:753 ;
    skos:definition "Subdivision CGoods produced in Japan from originating materials"@en-AU ;
    skos:narrower C1901A00006:746 ;
    skos:prefLabel "Subdivision S752"@en-AU ;
    dcat:accessURL "https://www.legislation.gov.au/C1901A00006/2024-07-01/2024-07-01/text/original/epub/OEBPS/document_2/document_2.html#_Toc172624507"^^xsd:anyURI .

C1901A00006:758 a legcons:Subdivision,
        skos:Concept,
        dcat:Resource ;
    rdfs:label "Subdivision S758"@en-AU ;
    rdfs:comment "Subdivision EConsignment - GraphNodeID: S758"@en-AU ;
    skos:broader C1901A00006:759 ;
    skos:definition "Subdivision EConsignment"@en-AU ;
    skos:narrower C1901A00006:746 ;
    skos:prefLabel "Subdivision S758"@en-AU ;
    dcat:accessURL "https://www.legislation.gov.au/C1901A00006/2024-07-01/2024-07-01/text/original/epub/OEBPS/document_2/document_2.html#_Toc172624513"^^xsd:anyURI .

C1901A00006:760 a legcons:Subdivision,
        skos:Concept,
        dcat:Resource ;
    rdfs:label "Subdivision S760"@en-AU ;
    rdfs:comment "Subdivision FRegulations - GraphNodeID: S760"@en-AU ;
    skos:broader C1901A00006:761 ;
    skos:definition "Subdivision FRegulations"@en-AU ;
    skos:narrower C1901A00006:746 ;
    skos:prefLabel "Subdivision S760"@en-AU ;
    dcat:accessURL "https://www.legislation.gov.au/C1901A00006/2024-07-01/2024-07-01/text/original/epub/OEBPS/document_2/document_2.html#_Toc172624515"^^xsd:anyURI .

C1901A00006:766 a legcons:Subdivision,
        skos:Concept,
        dcat:Resource ;
    rdfs:label "Subdivision S766"@en-AU ;
    rdfs:comment "Subdivision BGoods wholly obtained or produced in the territory of China - GraphNodeID: S766"@en-AU ;
    skos:broader C1901A00006:767 ;
    skos:definition "Subdivision BGoods wholly obtained or produced in the territory of China"@en-AU ;
    skos:narrower C1901A00006:762 ;
    skos:prefLabel "Subdivision S766"@en-AU ;
    dcat:accessURL "https://www.legislation.gov.au/C1901A00006/2024-07-01/2024-07-01/text/original/epub/OEBPS/document_2/document_2.html#_Toc172624521"^^xsd:anyURI .

C1901A00006:768 a legcons:Subdivision,
        skos:Concept,
        dcat:Resource ;
    rdfs:label "Subdivision S768"@en-AU ;
    rdfs:comment "Subdivision CGoods produced in China or in China and Australia from originating materials - GraphNodeID: S768"@en-AU ;
    skos:broader C1901A00006:769 ;
    skos:definition "Subdivision CGoods produced in China or in China and Australia from originating materials"@en-AU ;
    skos:narrower C1901A00006:762 ;
    skos:prefLabel "Subdivision S768"@en-AU ;
    dcat:accessURL "https://www.legislation.gov.au/C1901A00006/2024-07-01/2024-07-01/text/original/epub/OEBPS/document_2/document_2.html#_Toc172624523"^^xsd:anyURI .

C1901A00006:773 a legcons:Subdivision,
        skos:Concept,
        dcat:Resource ;
    rdfs:label "Subdivision S773"@en-AU ;
    rdfs:comment "Subdivision EGoods that are accessories spare parts or tools - GraphNodeID: S773"@en-AU ;
    skos:broader C1901A00006:774 ;
    skos:definition "Subdivision EGoods that are accessories spare parts or tools"@en-AU ;
    skos:narrower C1901A00006:762 ;
    skos:prefLabel "Subdivision S773"@en-AU ;
    dcat:accessURL "https://www.legislation.gov.au/C1901A00006/2024-07-01/2024-07-01/text/original/epub/OEBPS/document_2/document_2.html#_Toc172624528"^^xsd:anyURI .

C1901A00006:775 a legcons:Subdivision,
        skos:Concept,
        dcat:Resource ;
    rdfs:label "Subdivision S775"@en-AU ;
    rdfs:comment "Subdivision FNon qualifying operations - GraphNodeID: S775"@en-AU ;
    skos:broader C1901A00006:776 ;
    skos:definition "Subdivision FNon qualifying operations"@en-AU ;
    skos:narrower C1901A00006:762 ;
    skos:prefLabel "Subdivision S775"@en-AU ;
    dcat:accessURL "https://www.legislation.gov.au/C1901A00006/2024-07-01/2024-07-01/text/original/epub/OEBPS/document_2/document_2.html#_Toc172624530"^^xsd:anyURI .

C1901A00006:777 a legcons:Subdivision,
        skos:Concept,
        dcat:Resource ;
    rdfs:label "Subdivision S777"@en-AU ;
    rdfs:comment "Subdivision GConsignment - GraphNodeID: S777"@en-AU ;
    skos:broader C1901A00006:778 ;
    skos:definition "Subdivision GConsignment"@en-AU ;
    skos:narrower C1901A00006:762 ;
    skos:prefLabel "Subdivision S777"@en-AU ;
    dcat:accessURL "https://www.legislation.gov.au/C1901A00006/2024-07-01/2024-07-01/text/original/epub/OEBPS/document_2/document_2.html#_Toc172624532"^^xsd:anyURI .

C1901A00006:779 a legcons:Subdivision,
        skos:Concept,
        dcat:Resource ;
    rdfs:label "Subdivision S779"@en-AU ;
    rdfs:comment "Subdivision HRegulations - GraphNodeID: S779"@en-AU ;
    skos:broader C1901A00006:780 ;
    skos:definition "Subdivision HRegulations"@en-AU ;
    skos:narrower C1901A00006:762 ;
    skos:prefLabel "Subdivision S779"@en-AU ;
    dcat:accessURL "https://www.legislation.gov.au/C1901A00006/2024-07-01/2024-07-01/text/original/epub/OEBPS/document_2/document_2.html#_Toc172624534"^^xsd:anyURI .

C1901A00006:785 a legcons:Subdivision,
        skos:Concept,
        dcat:Resource ;
    rdfs:label "Subdivision S785"@en-AU ;
    rdfs:comment "Subdivision BGoods wholly obtained or produced entirely in Hong Kong China or in Hong Kong China and Australia - GraphNodeID: S785"@en-AU ;
    skos:broader C1901A00006:786 ;
    skos:definition "Subdivision BGoods wholly obtained or produced entirely in Hong Kong China or in Hong Kong China and Australia"@en-AU ;
    skos:narrower C1901A00006:781 ;
    skos:prefLabel "Subdivision S785"@en-AU ;
    dcat:accessURL "https://www.legislation.gov.au/C1901A00006/2024-07-01/2024-07-01/text/original/epub/OEBPS/document_2/document_2.html#_Toc172624540"^^xsd:anyURI .

C1901A00006:787 a legcons:Subdivision,
        skos:Concept,
        dcat:Resource ;
    rdfs:label "Subdivision S787"@en-AU ;
    rdfs:comment "Subdivision CGoods produced in Hong Kong China or in Hong Kong China and Australia from originating materials - GraphNodeID: S787"@en-AU ;
    skos:broader C1901A00006:788 ;
    skos:definition "Subdivision CGoods produced in Hong Kong China or in Hong Kong China and Australia from originating materials"@en-AU ;
    skos:narrower C1901A00006:781 ;
    skos:prefLabel "Subdivision S787"@en-AU ;
    dcat:accessURL "https://www.legislation.gov.au/C1901A00006/2024-07-01/2024-07-01/text/original/epub/OEBPS/document_2/document_2.html#_Toc172624542"^^xsd:anyURI .

C1901A00006:792 a legcons:Subdivision,
        skos:Concept,
        dcat:Resource ;
    rdfs:label "Subdivision S792"@en-AU ;
    rdfs:comment "Subdivision EGoods that are accessories spare parts tools or instructional or other information materials - GraphNodeID: S792"@en-AU ;
    skos:broader C1901A00006:793 ;
    skos:definition "Subdivision EGoods that are accessories spare parts tools or instructional or other information materials"@en-AU ;
    skos:narrower C1901A00006:781 ;
    skos:prefLabel "Subdivision S792"@en-AU ;
    dcat:accessURL "https://www.legislation.gov.au/C1901A00006/2024-07-01/2024-07-01/text/original/epub/OEBPS/document_2/document_2.html#_Toc172624547"^^xsd:anyURI .

C1901A00006:794 a legcons:Subdivision,
        skos:Concept,
        dcat:Resource ;
    rdfs:label "Subdivision S794"@en-AU ;
    rdfs:comment "Subdivision FConsignment - GraphNodeID: S794"@en-AU ;
    skos:broader C1901A00006:795 ;
    skos:definition "Subdivision FConsignment"@en-AU ;
    skos:narrower C1901A00006:781 ;
    skos:prefLabel "Subdivision S794"@en-AU ;
    dcat:accessURL "https://www.legislation.gov.au/C1901A00006/2024-07-01/2024-07-01/text/original/epub/OEBPS/document_2/document_2.html#_Toc172624549"^^xsd:anyURI .

C1901A00006:796 a legcons:Subdivision,
        skos:Concept,
        dcat:Resource ;
    rdfs:label "Subdivision S796"@en-AU ;
    rdfs:comment "Subdivision GRegulations - GraphNodeID: S796"@en-AU ;
    skos:broader C1901A00006:797 ;
    skos:definition "Subdivision GRegulations"@en-AU ;
    skos:narrower C1901A00006:781 ;
    skos:prefLabel "Subdivision S796"@en-AU ;
    dcat:accessURL "https://www.legislation.gov.au/C1901A00006/2024-07-01/2024-07-01/text/original/epub/OEBPS/document_2/document_2.html#_Toc172624551"^^xsd:anyURI .

C1901A00006:802 a legcons:Subdivision,
        skos:Concept,
        dcat:Resource ;
    rdfs:label "Subdivision S802"@en-AU ;
    rdfs:comment "Subdivision BGoods wholly obtained or produced in a Party - GraphNodeID: S802"@en-AU ;
    skos:broader C1901A00006:803 ;
    skos:definition "Subdivision BGoods wholly obtained or produced in a Party"@en-AU ;
    skos:narrower C1901A00006:798 ;
    skos:prefLabel "Subdivision S802"@en-AU ;
    dcat:accessURL "https://www.legislation.gov.au/C1901A00006/2024-07-01/2024-07-01/text/original/epub/OEBPS/document_2/document_2.html#_Toc172624557"^^xsd:anyURI .

C1901A00006:804 a legcons:Subdivision,
        skos:Concept,
        dcat:Resource ;
    rdfs:label "Subdivision S804"@en-AU ;
    rdfs:comment "Subdivision CGoods produced from originating materials - GraphNodeID: S804"@en-AU ;
    skos:broader C1901A00006:805 ;
    skos:definition "Subdivision CGoods produced from originating materials"@en-AU ;
    skos:narrower C1901A00006:798 ;
    skos:prefLabel "Subdivision S804"@en-AU ;
    dcat:accessURL "https://www.legislation.gov.au/C1901A00006/2024-07-01/2024-07-01/text/original/epub/OEBPS/document_2/document_2.html#_Toc172624559"^^xsd:anyURI .

C1901A00006:811 a legcons:Subdivision,
        skos:Concept,
        dcat:Resource ;
    rdfs:label "Subdivision S811"@en-AU ;
    rdfs:comment "Subdivision EConsignment - GraphNodeID: S811"@en-AU ;
    skos:broader C1901A00006:812 ;
    skos:definition "Subdivision EConsignment"@en-AU ;
    skos:narrower C1901A00006:798 ;
    skos:prefLabel "Subdivision S811"@en-AU ;
    dcat:accessURL "https://www.legislation.gov.au/C1901A00006/2024-07-01/2024-07-01/text/original/epub/OEBPS/document_2/document_2.html#_Toc172624566"^^xsd:anyURI .

C1901A00006:813 a legcons:Subdivision,
        skos:Concept,
        dcat:Resource ;
    rdfs:label "Subdivision S813"@en-AU ;
    rdfs:comment "Subdivision FRegulations - GraphNodeID: S813"@en-AU ;
    skos:broader C1901A00006:814 ;
    skos:definition "Subdivision FRegulations"@en-AU ;
    skos:narrower C1901A00006:798 ;
    skos:prefLabel "Subdivision S813"@en-AU ;
    dcat:accessURL "https://www.legislation.gov.au/C1901A00006/2024-07-01/2024-07-01/text/original/epub/OEBPS/document_2/document_2.html#_Toc172624568"^^xsd:anyURI .

C1901A00006:819 a legcons:Subdivision,
        skos:Concept,
        dcat:Resource ;
    rdfs:label "Subdivision S819"@en-AU ;
    rdfs:comment "Subdivision BGoods wholly obtained or produced in the United Kingdom or in the United Kingdom and Australia - GraphNodeID: S819"@en-AU ;
    skos:broader C1901A00006:820 ;
    skos:definition "Subdivision BGoods wholly obtained or produced in the United Kingdom or in the United Kingdom and Australia"@en-AU ;
    skos:narrower C1901A00006:815 ;
    skos:prefLabel "Subdivision S819"@en-AU ;
    dcat:accessURL "https://www.legislation.gov.au/C1901A00006/2024-07-01/2024-07-01/text/original/epub/OEBPS/document_2/document_2.html#_Toc172624574"^^xsd:anyURI .

C1901A00006:821 a legcons:Subdivision,
        skos:Concept,
        dcat:Resource ;
    rdfs:label "Subdivision S821"@en-AU ;
    rdfs:comment "Subdivision CGoods produced in the United Kingdom or in the United Kingdom and Australia from originating materials - GraphNodeID: S821"@en-AU ;
    skos:broader C1901A00006:822 ;
    skos:definition "Subdivision CGoods produced in the United Kingdom or in the United Kingdom and Australia from originating materials"@en-AU ;
    skos:narrower C1901A00006:815 ;
    skos:prefLabel "Subdivision S821"@en-AU ;
    dcat:accessURL "https://www.legislation.gov.au/C1901A00006/2024-07-01/2024-07-01/text/original/epub/OEBPS/document_2/document_2.html#_Toc172624576"^^xsd:anyURI .

C1901A00006:826 a legcons:Subdivision,
        skos:Concept,
        dcat:Resource ;
    rdfs:label "Subdivision S826"@en-AU ;
    rdfs:comment "Subdivision EGoods that are accessories spare parts tools or instructional or other information materials - GraphNodeID: S826"@en-AU ;
    skos:broader C1901A00006:827 ;
    skos:definition "Subdivision EGoods that are accessories spare parts tools or instructional or other information materials"@en-AU ;
    skos:narrower C1901A00006:815 ;
    skos:prefLabel "Subdivision S826"@en-AU ;
    dcat:accessURL "https://www.legislation.gov.au/C1901A00006/2024-07-01/2024-07-01/text/original/epub/OEBPS/document_2/document_2.html#_Toc172624581"^^xsd:anyURI .

C1901A00006:828 a legcons:Subdivision,
        skos:Concept,
        dcat:Resource ;
    rdfs:label "Subdivision S828"@en-AU ;
    rdfs:comment "Subdivision FConsignment - GraphNodeID: S828"@en-AU ;
    skos:broader C1901A00006:829 ;
    skos:definition "Subdivision FConsignment"@en-AU ;
    skos:narrower C1901A00006:815 ;
    skos:prefLabel "Subdivision S828"@en-AU ;
    dcat:accessURL "https://www.legislation.gov.au/C1901A00006/2024-07-01/2024-07-01/text/original/epub/OEBPS/document_2/document_2.html#_Toc172624583"^^xsd:anyURI .

C1901A00006:1015 a legcons:Subdivision,
        skos:Concept,
        dcat:Resource ;
    rdfs:label "Subdivision S1015"@en-AU ;
    rdfs:comment "Subdivision FDealing with things seized as evidential material - GraphNodeID: S1015"@en-AU ;
    skos:broader C1901A00006:1016,
        C1901A00006:1017 ;
    skos:definition "Subdivision FDealing with things seized as evidential material"@en-AU ;
    skos:narrower C1901A00006:954 ;
    skos:prefLabel "Subdivision S1015"@en-AU ;
    dcat:accessURL "https://www.legislation.gov.au/C1901A00006/2024-07-01/2024-07-01/text/original/epub/OEBPS/document_3/document_3.html#_Toc172627049"^^xsd:anyURI .

C1901A00006:1080 a legcons:Subdivision,
        skos:Concept,
        dcat:Resource ;
    rdfs:label "Subdivision S1080"@en-AU ;
    rdfs:comment "Subdivision HAInformation about people working in restricted areas or issued with security identification cards - GraphNodeID: S1080"@en-AU ;
    skos:broader C1901A00006:1081,
        C1901A00006:1082 ;
    skos:definition "Subdivision HAInformation about people working in restricted areas or issued with security identification cards"@en-AU ;
    skos:narrower C1901A00006:954 ;
    skos:prefLabel "Subdivision S1080"@en-AU ;
    dcat:accessURL "https://www.legislation.gov.au/C1901A00006/2024-07-01/2024-07-01/text/original/epub/OEBPS/document_3/document_3.html#_Toc172627114"^^xsd:anyURI .

C1901A00006:1155 a legcons:Subdivision,
        skos:Concept,
        dcat:Resource ;
    rdfs:label "Subdivision S1155"@en-AU ;
    rdfs:comment "Subdivision APreliminary - GraphNodeID: S1155"@en-AU ;
    skos:broader C1901A00006:1156,
        C1901A00006:1157 ;
    skos:definition "Subdivision APreliminary"@en-AU ;
    skos:narrower C1901A00006:1154 ;
    skos:prefLabel "Subdivision S1155"@en-AU ;
    dcat:accessURL "https://www.legislation.gov.au/C1901A00006/2024-07-01/2024-07-01/text/original/epub/OEBPS/document_3/document_3.html#_Toc172627189"^^xsd:anyURI .

C1901A00006:289 a legcons:Part,
        skos:Concept,
        dcat:Resource ;
    rdfs:label "Part P289"@en-AU ;
    rdfs:comment "Part VBInformation about persons departing Australia - GraphNodeID: P289"@en-AU ;
    skos:broader C1901A00006:290,
        C1901A00006:303 ;
    skos:definition "Part VBInformation about persons departing Australia"@en-AU ;
    skos:narrower C1901A00006:1 ;
    skos:prefLabel "Part P289"@en-AU ;
    dcat:accessURL "https://www.legislation.gov.au/C1901A00006/2024-07-01/2024-07-01/text/original/epub/OEBPS/document_1/document_1.html#_Toc172623263"^^xsd:anyURI .

C1901A00006:296 a legcons:Subdivision,
        skos:Concept,
        dcat:Resource ;
    rdfs:label "Subdivision S296"@en-AU ;
    rdfs:comment "Subdivision BReports on matters in approved statement - GraphNodeID: S296"@en-AU ;
    skos:broader C1901A00006:297,
        C1901A00006:298 ;
    skos:definition "Subdivision BReports on matters in approved statement"@en-AU ;
    skos:narrower C1901A00006:290 ;
    skos:prefLabel "Subdivision S296"@en-AU ;
    dcat:accessURL "https://www.legislation.gov.au/C1901A00006/2024-07-01/2024-07-01/text/original/epub/OEBPS/document_1/document_1.html#_Toc172623270"^^xsd:anyURI .

C1901A00006:320 a legcons:Subdivision,
        skos:Concept,
        dcat:Resource ;
    rdfs:label "Subdivision S320"@en-AU ;
    rdfs:comment "Subdivision APreliminary - GraphNodeID: S320"@en-AU ;
    skos:broader C1901A00006:321,
        C1901A00006:322 ;
    skos:definition "Subdivision APreliminary"@en-AU ;
    skos:narrower C1901A00006:319 ;
    skos:prefLabel "Subdivision S320"@en-AU ;
    dcat:accessURL "https://www.legislation.gov.au/C1901A00006/2024-07-01/2024-07-01/text/original/epub/OEBPS/document_1/document_1.html#_Toc172623294"^^xsd:anyURI .

C1901A00006:521 a legcons:Subdivision,
        skos:Concept,
        dcat:Resource ;
    rdfs:label "Subdivision S521"@en-AU ;
    rdfs:comment "Subdivision APreliminary - GraphNodeID: S521"@en-AU ;
    skos:broader C1901A00006:522,
        C1901A00006:523 ;
    skos:definition "Subdivision APreliminary"@en-AU ;
    skos:narrower C1901A00006:520 ;
    skos:prefLabel "Subdivision S521"@en-AU ;
    dcat:accessURL "https://www.legislation.gov.au/C1901A00006/2024-07-01/2024-07-01/text/original/epub/OEBPS/document_2/document_2.html#_Toc172624276"^^xsd:anyURI .

C1901A00006:528 a legcons:Subdivision,
        skos:Concept,
        dcat:Resource ;
    rdfs:label "Subdivision S528"@en-AU ;
    rdfs:comment "Subdivision DGoods produced in Singapore or in Singapore and Australia from non originating materials - GraphNodeID: S528"@en-AU ;
    skos:broader C1901A00006:529,
        C1901A00006:530 ;
    skos:definition "Subdivision DGoods produced in Singapore or in Singapore and Australia from non originating materials"@en-AU ;
    skos:narrower C1901A00006:520 ;
    skos:prefLabel "Subdivision S528"@en-AU ;
    dcat:accessURL "https://www.legislation.gov.au/C1901A00006/2024-07-01/2024-07-01/text/original/epub/OEBPS/document_2/document_2.html#_Toc172624283"^^xsd:anyURI .

C1901A00006:538 a legcons:Subdivision,
        skos:Concept,
        dcat:Resource ;
    rdfs:label "Subdivision S538"@en-AU ;
    rdfs:comment "Subdivision APreliminary - GraphNodeID: S538"@en-AU ;
    skos:broader C1901A00006:539,
        C1901A00006:540 ;
    skos:definition "Subdivision APreliminary"@en-AU ;
    skos:narrower C1901A00006:537 ;
    skos:prefLabel "Subdivision S538"@en-AU ;
    dcat:accessURL "https://www.legislation.gov.au/C1901A00006/2024-07-01/2024-07-01/text/original/epub/OEBPS/document_2/document_2.html#_Toc172624293"^^xsd:anyURI .

C1901A00006:556 a legcons:Subdivision,
        skos:Concept,
        dcat:Resource ;
    rdfs:label "Subdivision S556"@en-AU ;
    rdfs:comment "Subdivision APreliminary - GraphNodeID: S556"@en-AU ;
    skos:broader C1901A00006:557,
        C1901A00006:558 ;
    skos:definition "Subdivision APreliminary"@en-AU ;
    skos:narrower C1901A00006:555 ;
    skos:prefLabel "Subdivision S556"@en-AU ;
    dcat:accessURL "https://www.legislation.gov.au/C1901A00006/2024-07-01/2024-07-01/text/original/epub/OEBPS/document_2/document_2.html#_Toc172624311"^^xsd:anyURI .

C1901A00006:572 a legcons:Subdivision,
        skos:Concept,
        dcat:Resource ;
    rdfs:label "Subdivision S572"@en-AU ;
    rdfs:comment "Subdivision APreliminary - GraphNodeID: S572"@en-AU ;
    skos:broader C1901A00006:573,
        C1901A00006:574 ;
    skos:definition "Subdivision APreliminary"@en-AU ;
    skos:narrower C1901A00006:571 ;
    skos:prefLabel "Subdivision S572"@en-AU ;
    dcat:accessURL "https://www.legislation.gov.au/C1901A00006/2024-07-01/2024-07-01/text/original/epub/OEBPS/document_2/document_2.html#_Toc172624327"^^xsd:anyURI .

C1901A00006:579 a legcons:Subdivision,
        skos:Concept,
        dcat:Resource ;
    rdfs:label "Subdivision S579"@en-AU ;
    rdfs:comment "Subdivision DGoods produced in New Zealand or New Zealand and Australia from non originating materials - GraphNodeID: S579"@en-AU ;
    skos:broader C1901A00006:580,
        C1901A00006:581 ;
    skos:definition "Subdivision DGoods produced in New Zealand or New Zealand and Australia from non originating materials"@en-AU ;
    skos:narrower C1901A00006:571 ;
    skos:prefLabel "Subdivision S579"@en-AU ;
    dcat:accessURL "https://www.legislation.gov.au/C1901A00006/2024-07-01/2024-07-01/text/original/epub/OEBPS/document_2/document_2.html#_Toc172624334"^^xsd:anyURI .

C1901A00006:593 a legcons:Subdivision,
        skos:Concept,
        dcat:Resource ;
    rdfs:label "Subdivision S593"@en-AU ;
    rdfs:comment "Subdivision APreliminary - GraphNodeID: S593"@en-AU ;
    skos:broader C1901A00006:594,
        C1901A00006:595 ;
    skos:definition "Subdivision APreliminary"@en-AU ;
    skos:narrower C1901A00006:592 ;
    skos:prefLabel "Subdivision S593"@en-AU ;
    dcat:accessURL "https://www.legislation.gov.au/C1901A00006/2024-07-01/2024-07-01/text/original/epub/OEBPS/document_2/document_2.html#_Toc172624348"^^xsd:anyURI .

C1901A00006:600 a legcons:Subdivision,
        skos:Concept,
        dcat:Resource ;
    rdfs:label "Subdivision S600"@en-AU ;
    rdfs:comment "Subdivision DGoods produced in Peru or in Peru and Australia from non originating materials - GraphNodeID: S600"@en-AU ;
    skos:broader C1901A00006:601,
        C1901A00006:602 ;
    skos:definition "Subdivision DGoods produced in Peru or in Peru and Australia from non originating materials"@en-AU ;
    skos:narrower C1901A00006:592 ;
    skos:prefLabel "Subdivision S600"@en-AU ;
    dcat:accessURL "https://www.legislation.gov.au/C1901A00006/2024-07-01/2024-07-01/text/original/epub/OEBPS/document_2/document_2.html#_Toc172624355"^^xsd:anyURI .

C1901A00006:610 a legcons:Subdivision,
        skos:Concept,
        dcat:Resource ;
    rdfs:label "Subdivision S610"@en-AU ;
    rdfs:comment "Subdivision APreliminary - GraphNodeID: S610"@en-AU ;
    skos:broader C1901A00006:611,
        C1901A00006:612 ;
    skos:definition "Subdivision APreliminary"@en-AU ;
    skos:narrower C1901A00006:609 ;
    skos:prefLabel "Subdivision S610"@en-AU ;
    dcat:accessURL "https://www.legislation.gov.au/C1901A00006/2024-07-01/2024-07-01/text/original/epub/OEBPS/document_2/document_2.html#_Toc172624365"^^xsd:anyURI .

C1901A00006:617 a legcons:Subdivision,
        skos:Concept,
        dcat:Resource ;
    rdfs:label "Subdivision S617"@en-AU ;
    rdfs:comment "Subdivision DGoods produced in Chile or Chile and Australia from non originating materials - GraphNodeID: S617"@en-AU ;
    skos:broader C1901A00006:618,
        C1901A00006:619 ;
    skos:definition "Subdivision DGoods produced in Chile or Chile and Australia from non originating materials"@en-AU ;
    skos:narrower C1901A00006:609 ;
    skos:prefLabel "Subdivision S617"@en-AU ;
    dcat:accessURL "https://www.legislation.gov.au/C1901A00006/2024-07-01/2024-07-01/text/original/epub/OEBPS/document_2/document_2.html#_Toc172624372"^^xsd:anyURI .

C1901A00006:629 a legcons:Subdivision,
        skos:Concept,
        dcat:Resource ;
    rdfs:label "Subdivision S629"@en-AU ;
    rdfs:comment "Subdivision APreliminary - GraphNodeID: S629"@en-AU ;
    skos:broader C1901A00006:630,
        C1901A00006:631 ;
    skos:definition "Subdivision APreliminary"@en-AU ;
    skos:narrower C1901A00006:628 ;
    skos:prefLabel "Subdivision S629"@en-AU ;
    dcat:accessURL "https://www.legislation.gov.au/C1901A00006/2024-07-01/2024-07-01/text/original/epub/OEBPS/document_2/document_2.html#_Toc172624384"^^xsd:anyURI .

C1901A00006:647 a legcons:Subdivision,
        skos:Concept,
        dcat:Resource ;
    rdfs:label "Subdivision S647"@en-AU ;
    rdfs:comment "Subdivision APreliminary - GraphNodeID: S647"@en-AU ;
    skos:broader C1901A00006:648,
        C1901A00006:649 ;
    skos:definition "Subdivision APreliminary"@en-AU ;
    skos:narrower C1901A00006:646 ;
    skos:prefLabel "Subdivision S647"@en-AU ;
    dcat:accessURL "https://www.legislation.gov.au/C1901A00006/2024-07-01/2024-07-01/text/original/epub/OEBPS/document_2/document_2.html#_Toc172624402"^^xsd:anyURI .

C1901A00006:654 a legcons:Subdivision,
        skos:Concept,
        dcat:Resource ;
    rdfs:label "Subdivision S654"@en-AU ;
    rdfs:comment "Subdivision DGoods produced from non originating materials - GraphNodeID: S654"@en-AU ;
    skos:broader C1901A00006:655,
        C1901A00006:656 ;
    skos:definition "Subdivision DGoods produced from non originating materials"@en-AU ;
    skos:narrower C1901A00006:646 ;
    skos:prefLabel "Subdivision S654"@en-AU ;
    dcat:accessURL "https://www.legislation.gov.au/C1901A00006/2024-07-01/2024-07-01/text/original/epub/OEBPS/document_2/document_2.html#_Toc172624409"^^xsd:anyURI .

C1901A00006:664 a legcons:Subdivision,
        skos:Concept,
        dcat:Resource ;
    rdfs:label "Subdivision S664"@en-AU ;
    rdfs:comment "Subdivision APreliminary - GraphNodeID: S664"@en-AU ;
    skos:broader C1901A00006:665,
        C1901A00006:666 ;
    skos:definition "Subdivision APreliminary"@en-AU ;
    skos:narrower C1901A00006:663 ;
    skos:prefLabel "Subdivision S664"@en-AU ;
    dcat:accessURL "https://www.legislation.gov.au/C1901A00006/2024-07-01/2024-07-01/text/original/epub/OEBPS/document_2/document_2.html#_Toc172624419"^^xsd:anyURI .

C1901A00006:671 a legcons:Subdivision,
        skos:Concept,
        dcat:Resource ;
    rdfs:label "Subdivision S671"@en-AU ;
    rdfs:comment "Subdivision DGoods produced from non originating materials - GraphNodeID: S671"@en-AU ;
    skos:broader C1901A00006:672,
        C1901A00006:673 ;
    skos:definition "Subdivision DGoods produced from non originating materials"@en-AU ;
    skos:narrower C1901A00006:663 ;
    skos:prefLabel "Subdivision S671"@en-AU ;
    dcat:accessURL "https://www.legislation.gov.au/C1901A00006/2024-07-01/2024-07-01/text/original/epub/OEBPS/document_2/document_2.html#_Toc172624426"^^xsd:anyURI .

C1901A00006:681 a legcons:Subdivision,
        skos:Concept,
        dcat:Resource ;
    rdfs:label "Subdivision S681"@en-AU ;
    rdfs:comment "Subdivision APreliminary - GraphNodeID: S681"@en-AU ;
    skos:broader C1901A00006:682,
        C1901A00006:683 ;
    skos:definition "Subdivision APreliminary"@en-AU ;
    skos:narrower C1901A00006:680 ;
    skos:prefLabel "Subdivision S681"@en-AU ;
    dcat:accessURL "https://www.legislation.gov.au/C1901A00006/2024-07-01/2024-07-01/text/original/epub/OEBPS/document_2/document_2.html#_Toc172624436"^^xsd:anyURI .

C1901A00006:699 a legcons:Subdivision,
        skos:Concept,
        dcat:Resource ;
    rdfs:label "Subdivision S699"@en-AU ;
    rdfs:comment "Subdivision APreliminary - GraphNodeID: S699"@en-AU ;
    skos:broader C1901A00006:700,
        C1901A00006:701 ;
    skos:definition "Subdivision APreliminary"@en-AU ;
    skos:narrower C1901A00006:698 ;
    skos:prefLabel "Subdivision S699"@en-AU ;
    dcat:accessURL "https://www.legislation.gov.au/C1901A00006/2024-07-01/2024-07-01/text/original/epub/OEBPS/document_2/document_2.html#_Toc172624454"^^xsd:anyURI .

C1901A00006:706 a legcons:Subdivision,
        skos:Concept,
        dcat:Resource ;
    rdfs:label "Subdivision S706"@en-AU ;
    rdfs:comment "Subdivision DGoods produced in Indonesia or in Indonesia and Australia from non originating materials - GraphNodeID: S706"@en-AU ;
    skos:broader C1901A00006:707,
        C1901A00006:708 ;
    skos:definition "Subdivision DGoods produced in Indonesia or in Indonesia and Australia from non originating materials"@en-AU ;
    skos:narrower C1901A00006:698 ;
    skos:prefLabel "Subdivision S706"@en-AU ;
    dcat:accessURL "https://www.legislation.gov.au/C1901A00006/2024-07-01/2024-07-01/text/original/epub/OEBPS/document_2/document_2.html#_Toc172624461"^^xsd:anyURI .

C1901A00006:709 a legcons:Subdivision,
        skos:Concept,
        dcat:Resource ;
    rdfs:label "Subdivision S709"@en-AU ;
    rdfs:comment "Subdivision EConsignment and exhibition - GraphNodeID: S709"@en-AU ;
    skos:broader C1901A00006:710,
        C1901A00006:711 ;
    skos:definition "Subdivision EConsignment and exhibition"@en-AU ;
    skos:narrower C1901A00006:698 ;
    skos:prefLabel "Subdivision S709"@en-AU ;
    dcat:accessURL "https://www.legislation.gov.au/C1901A00006/2024-07-01/2024-07-01/text/original/epub/OEBPS/document_2/document_2.html#_Toc172624464"^^xsd:anyURI .

C1901A00006:715 a legcons:Subdivision,
        skos:Concept,
        dcat:Resource ;
    rdfs:label "Subdivision S715"@en-AU ;
    rdfs:comment "Subdivision APreliminary - GraphNodeID: S715"@en-AU ;
    skos:broader C1901A00006:716,
        C1901A00006:717 ;
    skos:definition "Subdivision APreliminary"@en-AU ;
    skos:narrower C1901A00006:714 ;
    skos:prefLabel "Subdivision S715"@en-AU ;
    dcat:accessURL "https://www.legislation.gov.au/C1901A00006/2024-07-01/2024-07-01/text/original/epub/OEBPS/document_2/document_2.html#_Toc172624470"^^xsd:anyURI .

C1901A00006:722 a legcons:Subdivision,
        skos:Concept,
        dcat:Resource ;
    rdfs:label "Subdivision S722"@en-AU ;
    rdfs:comment "Subdivision DGoods produced in Korea or in Korea and Australia from non originating materials - GraphNodeID: S722"@en-AU ;
    skos:broader C1901A00006:723,
        C1901A00006:724 ;
    skos:definition "Subdivision DGoods produced in Korea or in Korea and Australia from non originating materials"@en-AU ;
    skos:narrower C1901A00006:714 ;
    skos:prefLabel "Subdivision S722"@en-AU ;
    dcat:accessURL "https://www.legislation.gov.au/C1901A00006/2024-07-01/2024-07-01/text/original/epub/OEBPS/document_2/document_2.html#_Toc172624477"^^xsd:anyURI .

C1901A00006:732 a legcons:Subdivision,
        skos:Concept,
        dcat:Resource ;
    rdfs:label "Subdivision S732"@en-AU ;
    rdfs:comment "Subdivision APreliminary - GraphNodeID: S732"@en-AU ;
    skos:broader C1901A00006:733,
        C1901A00006:734 ;
    skos:definition "Subdivision APreliminary"@en-AU ;
    skos:narrower C1901A00006:731 ;
    skos:prefLabel "Subdivision S732"@en-AU ;
    dcat:accessURL "https://www.legislation.gov.au/C1901A00006/2024-07-01/2024-07-01/text/original/epub/OEBPS/document_2/document_2.html#_Toc172624487"^^xsd:anyURI .

C1901A00006:737 a legcons:Subdivision,
        skos:Concept,
        dcat:Resource ;
    rdfs:label "Subdivision S737"@en-AU ;
    rdfs:comment "Subdivision CGoods produced in India or in India and Australia from non originating materials - GraphNodeID: S737"@en-AU ;
    skos:broader C1901A00006:738,
        C1901A00006:739 ;
    skos:definition "Subdivision CGoods produced in India or in India and Australia from non originating materials"@en-AU ;
    skos:narrower C1901A00006:731 ;
    skos:prefLabel "Subdivision S737"@en-AU ;
    dcat:accessURL "https://www.legislation.gov.au/C1901A00006/2024-07-01/2024-07-01/text/original/epub/OEBPS/document_2/document_2.html#_Toc172624492"^^xsd:anyURI .

C1901A00006:747 a legcons:Subdivision,
        skos:Concept,
        dcat:Resource ;
    rdfs:label "Subdivision S747"@en-AU ;
    rdfs:comment "Subdivision APreliminary - GraphNodeID: S747"@en-AU ;
    skos:broader C1901A00006:748,
        C1901A00006:749 ;
    skos:definition "Subdivision APreliminary"@en-AU ;
    skos:narrower C1901A00006:746 ;
    skos:prefLabel "Subdivision S747"@en-AU ;
    dcat:accessURL "https://www.legislation.gov.au/C1901A00006/2024-07-01/2024-07-01/text/original/epub/OEBPS/document_2/document_2.html#_Toc172624502"^^xsd:anyURI .

C1901A00006:763 a legcons:Subdivision,
        skos:Concept,
        dcat:Resource ;
    rdfs:label "Subdivision S763"@en-AU ;
    rdfs:comment "Subdivision APreliminary - GraphNodeID: S763"@en-AU ;
    skos:broader C1901A00006:764,
        C1901A00006:765 ;
    skos:definition "Subdivision APreliminary"@en-AU ;
    skos:narrower C1901A00006:762 ;
    skos:prefLabel "Subdivision S763"@en-AU ;
    dcat:accessURL "https://www.legislation.gov.au/C1901A00006/2024-07-01/2024-07-01/text/original/epub/OEBPS/document_2/document_2.html#_Toc172624518"^^xsd:anyURI .

C1901A00006:770 a legcons:Subdivision,
        skos:Concept,
        dcat:Resource ;
    rdfs:label "Subdivision S770"@en-AU ;
    rdfs:comment "Subdivision DGoods produced in China or in China and Australia from non originating materials - GraphNodeID: S770"@en-AU ;
    skos:broader C1901A00006:771,
        C1901A00006:772 ;
    skos:definition "Subdivision DGoods produced in China or in China and Australia from non originating materials"@en-AU ;
    skos:narrower C1901A00006:762 ;
    skos:prefLabel "Subdivision S770"@en-AU ;
    dcat:accessURL "https://www.legislation.gov.au/C1901A00006/2024-07-01/2024-07-01/text/original/epub/OEBPS/document_2/document_2.html#_Toc172624525"^^xsd:anyURI .

C1901A00006:782 a legcons:Subdivision,
        skos:Concept,
        dcat:Resource ;
    rdfs:label "Subdivision S782"@en-AU ;
    rdfs:comment "Subdivision APreliminary - GraphNodeID: S782"@en-AU ;
    skos:broader C1901A00006:783,
        C1901A00006:784 ;
    skos:definition "Subdivision APreliminary"@en-AU ;
    skos:narrower C1901A00006:781 ;
    skos:prefLabel "Subdivision S782"@en-AU ;
    dcat:accessURL "https://www.legislation.gov.au/C1901A00006/2024-07-01/2024-07-01/text/original/epub/OEBPS/document_2/document_2.html#_Toc172624537"^^xsd:anyURI .

C1901A00006:789 a legcons:Subdivision,
        skos:Concept,
        dcat:Resource ;
    rdfs:label "Subdivision S789"@en-AU ;
    rdfs:comment "Subdivision DGoods produced in Hong Kong China or in Hong Kong China and Australia from non originating materials - GraphNodeID: S789"@en-AU ;
    skos:broader C1901A00006:790,
        C1901A00006:791 ;
    skos:definition "Subdivision DGoods produced in Hong Kong China or in Hong Kong China and Australia from non originating materials"@en-AU ;
    skos:narrower C1901A00006:781 ;
    skos:prefLabel "Subdivision S789"@en-AU ;
    dcat:accessURL "https://www.legislation.gov.au/C1901A00006/2024-07-01/2024-07-01/text/original/epub/OEBPS/document_2/document_2.html#_Toc172624544"^^xsd:anyURI .

C1901A00006:799 a legcons:Subdivision,
        skos:Concept,
        dcat:Resource ;
    rdfs:label "Subdivision S799"@en-AU ;
    rdfs:comment "Subdivision APreliminary - GraphNodeID: S799"@en-AU ;
    skos:broader C1901A00006:800,
        C1901A00006:801 ;
    skos:definition "Subdivision APreliminary"@en-AU ;
    skos:narrower C1901A00006:798 ;
    skos:prefLabel "Subdivision S799"@en-AU ;
    dcat:accessURL "https://www.legislation.gov.au/C1901A00006/2024-07-01/2024-07-01/text/original/epub/OEBPS/document_2/document_2.html#_Toc172624554"^^xsd:anyURI .

C1901A00006:816 a legcons:Subdivision,
        skos:Concept,
        dcat:Resource ;
    rdfs:label "Subdivision S816"@en-AU ;
    rdfs:comment "Subdivision APreliminary - GraphNodeID: S816"@en-AU ;
    skos:broader C1901A00006:817,
        C1901A00006:818 ;
    skos:definition "Subdivision APreliminary"@en-AU ;
    skos:narrower C1901A00006:815 ;
    skos:prefLabel "Subdivision S816"@en-AU ;
    dcat:accessURL "https://www.legislation.gov.au/C1901A00006/2024-07-01/2024-07-01/text/original/epub/OEBPS/document_2/document_2.html#_Toc172624571"^^xsd:anyURI .

C1901A00006:823 a legcons:Subdivision,
        skos:Concept,
        dcat:Resource ;
    rdfs:label "Subdivision S823"@en-AU ;
    rdfs:comment "Subdivision DGoods produced in the United Kingdom or in the United Kingdom and Australia from non originating materials - GraphNodeID: S823"@en-AU ;
    skos:broader C1901A00006:824,
        C1901A00006:825 ;
    skos:definition "Subdivision DGoods produced in the United Kingdom or in the United Kingdom and Australia from non originating materials"@en-AU ;
    skos:narrower C1901A00006:815 ;
    skos:prefLabel "Subdivision S823"@en-AU ;
    dcat:accessURL "https://www.legislation.gov.au/C1901A00006/2024-07-01/2024-07-01/text/original/epub/OEBPS/document_2/document_2.html#_Toc172624578"^^xsd:anyURI .

C1901A00006:871 a legcons:Division,
        skos:Concept,
        dcat:Resource ;
    rdfs:label "Division D871"@en-AU ;
    rdfs:comment "Division 2 Trusted trader agreement - GraphNodeID: D871"@en-AU ;
    skos:broader C1901A00006:872,
        C1901A00006:875 ;
    skos:definition "Division 2 Trusted trader agreement"@en-AU ;
    skos:narrower C1901A00006:868 ;
    skos:prefLabel "Division D871"@en-AU ;
    dcat:accessURL "https://www.legislation.gov.au/C1901A00006/2024-07-01/2024-07-01/text/original/epub/OEBPS/document_2/document_2.html#_Toc172624626"^^xsd:anyURI .

C1901A00006:872 a legcons:Subdivision,
        skos:Concept,
        dcat:Resource ;
    rdfs:label "Subdivision S872"@en-AU ;
    rdfs:comment "Subdivision AEntry into trusted trader agreement - GraphNodeID: S872"@en-AU ;
    skos:broader C1901A00006:873,
        C1901A00006:874 ;
    skos:definition "Subdivision AEntry into trusted trader agreement"@en-AU ;
    skos:narrower C1901A00006:871 ;
    skos:prefLabel "Subdivision S872"@en-AU ;
    dcat:accessURL "https://www.legislation.gov.au/C1901A00006/2024-07-01/2024-07-01/text/original/epub/OEBPS/document_2/document_2.html#_Toc172624627"^^xsd:anyURI .

C1901A00006:999 a legcons:Subdivision,
        skos:Concept,
        dcat:Resource ;
    rdfs:label "Subdivision S999"@en-AU ;
    rdfs:comment "Subdivision DASeizure of certain goods in transit - GraphNodeID: S999"@en-AU ;
    skos:broader C1901A00006:1000,
        C1901A00006:1001 ;
    skos:definition "Subdivision DASeizure of certain goods in transit"@en-AU ;
    skos:narrower C1901A00006:954 ;
    skos:prefLabel "Subdivision S999"@en-AU ;
    dcat:accessURL "https://www.legislation.gov.au/C1901A00006/2024-07-01/2024-07-01/text/original/epub/OEBPS/document_3/document_3.html#_Toc172627033"^^xsd:anyURI .

C1901A00006:1121 a legcons:Subdivision,
        skos:Concept,
        dcat:Resource ;
    rdfs:label "Subdivision S1121"@en-AU ;
    rdfs:comment "Subdivision BDetention and external search of suspects - GraphNodeID: S1121"@en-AU ;
    skos:broader C1901A00006:1122,
        C1901A00006:1123,
        C1901A00006:1124 ;
    skos:definition "Subdivision BDetention and external search of suspects"@en-AU ;
    skos:narrower C1901A00006:1115 ;
    skos:prefLabel "Subdivision S1121"@en-AU ;
    dcat:accessURL "https://www.legislation.gov.au/C1901A00006/2024-07-01/2024-07-01/text/original/epub/OEBPS/document_3/document_3.html#_Toc172627155"^^xsd:anyURI .

C1901A00006:1154 a legcons:Division,
        skos:Concept,
        dcat:Resource ;
    rdfs:label "Division D1154"@en-AU ;
    rdfs:comment "Division 1 BADetention and search of persons for purposes of law enforcement co operation - GraphNodeID: D1154"@en-AU ;
    skos:broader C1901A00006:1155,
        C1901A00006:1158,
        C1901A00006:1162 ;
    skos:definition "Division 1 BADetention and search of persons for purposes of law enforcement co operation"@en-AU ;
    skos:narrower C1901A00006:953 ;
    skos:prefLabel "Division D1154"@en-AU ;
    dcat:accessURL "https://www.legislation.gov.au/C1901A00006/2024-07-01/2024-07-01/text/original/epub/OEBPS/document_3/document_3.html#_Toc172627188"^^xsd:anyURI .

C1901A00006:1158 a legcons:Subdivision,
        skos:Concept,
        dcat:Resource ;
    rdfs:label "Subdivision S1158"@en-AU ;
    rdfs:comment "Subdivision BPowers to detain - GraphNodeID: S1158"@en-AU ;
    skos:broader C1901A00006:1159,
        C1901A00006:1160,
        C1901A00006:1161 ;
    skos:definition "Subdivision BPowers to detain"@en-AU ;
    skos:narrower C1901A00006:1154 ;
    skos:prefLabel "Subdivision S1158"@en-AU ;
    dcat:accessURL "https://www.legislation.gov.au/C1901A00006/2024-07-01/2024-07-01/text/original/epub/OEBPS/document_3/document_3.html#_Toc172627192"^^xsd:anyURI .

C1901A00006:127 a legcons:Subdivision,
        skos:Concept,
        dcat:Resource ;
    rdfs:label "Subdivision S127"@en-AU ;
    rdfs:comment "Subdivision AAInformation and grant of authority to deal with Subdivision AA goods - GraphNodeID: S127"@en-AU ;
    skos:broader C1901A00006:128,
        C1901A00006:129,
        C1901A00006:130 ;
    skos:definition "Subdivision AAInformation and grant of authority to deal with Subdivision AA goods"@en-AU ;
    skos:narrower C1901A00006:120 ;
    skos:prefLabel "Subdivision S127"@en-AU ;
    dcat:accessURL "https://www.legislation.gov.au/C1901A00006/2024-07-01/2024-07-01/text/original/epub/OEBPS/document_1/document_1.html#_Toc172623101"^^xsd:anyURI .

C1901A00006:1326 a legcons:Volume,
        skos:Concept,
        dcat:Resource ;
    rdfs:label "Volume V1326"@en-AU ;
    rdfs:comment "Volume 4 - GraphNodeID: V1326"@en-AU ;
    skos:broader C1901A00006:1327,
        C1901A00006:1508,
        C1901A00006:1517,
        C1901A00006:1528 ;
    skos:definition "Volume 4"@en-AU ;
    skos:prefLabel "Volume V1326"@en-AU ;
    dcat:accessURL "https://www.legislation.gov.au/C1901A00006/2024-07-01/2024-07-01/text/original/epub/OEBPS/document_4/document_4.html"^^xsd:anyURI .

C1901A00006:290 a legcons:Division,
        skos:Concept,
        dcat:Resource ;
    rdfs:label "Division D290"@en-AU ;
    rdfs:comment "Division 1 Reports on departing persons - GraphNodeID: D290"@en-AU ;
    skos:broader C1901A00006:291,
        C1901A00006:296,
        C1901A00006:299 ;
    skos:definition "Division 1 Reports on departing persons"@en-AU ;
    skos:narrower C1901A00006:289 ;
    skos:prefLabel "Division D290"@en-AU ;
    dcat:accessURL "https://www.legislation.gov.au/C1901A00006/2024-07-01/2024-07-01/text/original/epub/OEBPS/document_1/document_1.html#_Toc172623264"^^xsd:anyURI .

C1901A00006:319 a legcons:Division,
        skos:Concept,
        dcat:Resource ;
    rdfs:label "Division D319"@en-AU ;
    rdfs:comment "Division 2 Entry and clearance of goods for export - GraphNodeID: D319"@en-AU ;
    skos:broader C1901A00006:320,
        C1901A00006:323,
        C1901A00006:327 ;
    skos:definition "Division 2 Entry and clearance of goods for export"@en-AU ;
    skos:narrower C1901A00006:305 ;
    skos:prefLabel "Division D319"@en-AU ;
    dcat:accessURL "https://www.legislation.gov.au/C1901A00006/2024-07-01/2024-07-01/text/original/epub/OEBPS/document_1/document_1.html#_Toc172623293"^^xsd:anyURI .

C1901A00006:323 a legcons:Subdivision,
        skos:Concept,
        dcat:Resource ;
    rdfs:label "Subdivision S323"@en-AU ;
    rdfs:comment "Subdivision BExport declarations - GraphNodeID: S323"@en-AU ;
    skos:broader C1901A00006:324,
        C1901A00006:325,
        C1901A00006:326 ;
    skos:definition "Subdivision BExport declarations"@en-AU ;
    skos:narrower C1901A00006:319 ;
    skos:prefLabel "Subdivision S323"@en-AU ;
    dcat:accessURL "https://www.legislation.gov.au/C1901A00006/2024-07-01/2024-07-01/text/original/epub/OEBPS/document_1/document_1.html#_Toc172623297"^^xsd:anyURI .

C1901A00006:636 a legcons:Subdivision,
        skos:Concept,
        dcat:Resource ;
    rdfs:label "Subdivision S636"@en-AU ;
    rdfs:comment "Subdivision DGoods produced from non originating materials - GraphNodeID: S636"@en-AU ;
    skos:broader C1901A00006:637,
        C1901A00006:638,
        C1901A00006:639 ;
    skos:definition "Subdivision DGoods produced from non originating materials"@en-AU ;
    skos:narrower C1901A00006:628 ;
    skos:prefLabel "Subdivision S636"@en-AU ;
    dcat:accessURL "https://www.legislation.gov.au/C1901A00006/2024-07-01/2024-07-01/text/original/epub/OEBPS/document_2/document_2.html#_Toc172624391"^^xsd:anyURI .

C1901A00006:688 a legcons:Subdivision,
        skos:Concept,
        dcat:Resource ;
    rdfs:label "Subdivision S688"@en-AU ;
    rdfs:comment "Subdivision DGoods produced in Malaysia or in Malaysia and Australia from non originating materials - GraphNodeID: S688"@en-AU ;
    skos:broader C1901A00006:689,
        C1901A00006:690,
        C1901A00006:691 ;
    skos:definition "Subdivision DGoods produced in Malaysia or in Malaysia and Australia from non originating materials"@en-AU ;
    skos:narrower C1901A00006:680 ;
    skos:prefLabel "Subdivision S688"@en-AU ;
    dcat:accessURL "https://www.legislation.gov.au/C1901A00006/2024-07-01/2024-07-01/text/original/epub/OEBPS/document_2/document_2.html#_Toc172624443"^^xsd:anyURI .

C1901A00006:727 a legcons:Subdivision,
        skos:Concept,
        dcat:Resource ;
    rdfs:label "Subdivision S727"@en-AU ;
    rdfs:comment "Subdivision FOther matters - GraphNodeID: S727"@en-AU ;
    skos:broader C1901A00006:728,
        C1901A00006:729,
        C1901A00006:730 ;
    skos:definition "Subdivision FOther matters"@en-AU ;
    skos:narrower C1901A00006:714 ;
    skos:prefLabel "Subdivision S727"@en-AU ;
    dcat:accessURL "https://www.legislation.gov.au/C1901A00006/2024-07-01/2024-07-01/text/original/epub/OEBPS/document_2/document_2.html#_Toc172624482"^^xsd:anyURI .

C1901A00006:74 a legcons:Division,
        skos:Concept,
        dcat:Resource ;
    rdfs:label "Division D74"@en-AU ;
    rdfs:comment "Division 3 The report of the cargo - GraphNodeID: D74"@en-AU ;
    skos:broader C1901A00006:113,
        C1901A00006:75,
        C1901A00006:99 ;
    skos:definition "Division 3 The report of the cargo"@en-AU ;
    skos:narrower C1901A00006:54 ;
    skos:prefLabel "Division D74"@en-AU ;
    dcat:accessURL "https://www.legislation.gov.au/C1901A00006/2024-07-01/2024-07-01/text/original/epub/OEBPS/document_1/document_1.html#_Toc172623048"^^xsd:anyURI .

C1901A00006:754 a legcons:Subdivision,
        skos:Concept,
        dcat:Resource ;
    rdfs:label "Subdivision S754"@en-AU ;
    rdfs:comment "Subdivision DGoods produced in Japan or in Japan and Australia from non originating materials - GraphNodeID: S754"@en-AU ;
    skos:broader C1901A00006:755,
        C1901A00006:756,
        C1901A00006:757 ;
    skos:definition "Subdivision DGoods produced in Japan or in Japan and Australia from non originating materials"@en-AU ;
    skos:narrower C1901A00006:746 ;
    skos:prefLabel "Subdivision S754"@en-AU ;
    dcat:accessURL "https://www.legislation.gov.au/C1901A00006/2024-07-01/2024-07-01/text/original/epub/OEBPS/document_2/document_2.html#_Toc172624509"^^xsd:anyURI .

C1901A00006:1116 a legcons:Subdivision,
        skos:Concept,
        dcat:Resource ;
    rdfs:label "Subdivision S1116"@en-AU ;
    rdfs:comment "Subdivision ADetention and frisk search of suspects - GraphNodeID: S1116"@en-AU ;
    skos:broader C1901A00006:1117,
        C1901A00006:1118,
        C1901A00006:1119,
        C1901A00006:1120 ;
    skos:definition "Subdivision ADetention and frisk search of suspects"@en-AU ;
    skos:narrower C1901A00006:1115 ;
    skos:prefLabel "Subdivision S1116"@en-AU ;
    dcat:accessURL "https://www.legislation.gov.au/C1901A00006/2024-07-01/2024-07-01/text/original/epub/OEBPS/document_3/document_3.html#_Toc172627150"^^xsd:anyURI .

C1901A00006:1149 a legcons:Subdivision,
        skos:Concept,
        dcat:Resource ;
    rdfs:label "Subdivision S1149"@en-AU ;
    rdfs:comment "Subdivision EMedical practitioners - GraphNodeID: S1149"@en-AU ;
    skos:broader C1901A00006:1150,
        C1901A00006:1151,
        C1901A00006:1152,
        C1901A00006:1153 ;
    skos:definition "Subdivision EMedical practitioners"@en-AU ;
    skos:narrower C1901A00006:1115 ;
    skos:prefLabel "Subdivision S1149"@en-AU ;
    dcat:accessURL "https://www.legislation.gov.au/C1901A00006/2024-07-01/2024-07-01/text/original/epub/OEBPS/document_3/document_3.html#_Toc172627183"^^xsd:anyURI .

C1901A00006:1332 a legcons:Subdivision,
        skos:Concept,
        dcat:Resource ;
    rdfs:label "Subdivision S1332"@en-AU ;
    rdfs:comment "Subdivision BAnti Dumping Commission - GraphNodeID: S1332"@en-AU ;
    skos:broader C1901A00006:1333,
        C1901A00006:1334,
        C1901A00006:1335,
        C1901A00006:1336 ;
    skos:definition "Subdivision BAnti Dumping Commission"@en-AU ;
    skos:narrower C1901A00006:1329 ;
    skos:prefLabel "Subdivision S1332"@en-AU ;
    dcat:accessURL "https://www.legislation.gov.au/C1901A00006/2024-07-01/2024-07-01/text/original/epub/OEBPS/document_4/document_4.html#_Toc172628766"^^xsd:anyURI .

C1901A00006:1465 a legcons:Division,
        skos:Concept,
        dcat:Resource ;
    rdfs:label "Division D1465"@en-AU ;
    rdfs:comment "Division 9 Review by Review Panel - GraphNodeID: D1465"@en-AU ;
    skos:broader C1901A00006:1466,
        C1901A00006:1473,
        C1901A00006:1488,
        C1901A00006:1504 ;
    skos:definition "Division 9 Review by Review Panel"@en-AU ;
    skos:narrower C1901A00006:1327 ;
    skos:prefLabel "Division D1465"@en-AU ;
    dcat:accessURL "https://www.legislation.gov.au/C1901A00006/2024-07-01/2024-07-01/text/original/epub/OEBPS/document_4/document_4.html#_Toc172628899"^^xsd:anyURI .

C1901A00006:291 a legcons:Subdivision,
        skos:Concept,
        dcat:Resource ;
    rdfs:label "Subdivision S291"@en-AU ;
    rdfs:comment "Subdivision AReports on departing persons - GraphNodeID: S291"@en-AU ;
    skos:broader C1901A00006:292,
        C1901A00006:293,
        C1901A00006:294,
        C1901A00006:295 ;
    skos:definition "Subdivision AReports on departing persons"@en-AU ;
    skos:narrower C1901A00006:290 ;
    skos:prefLabel "Subdivision S291"@en-AU ;
    dcat:accessURL "https://www.legislation.gov.au/C1901A00006/2024-07-01/2024-07-01/text/original/epub/OEBPS/document_1/document_1.html#_Toc172623265"^^xsd:anyURI .

C1901A00006:55 a legcons:Division,
        skos:Concept,
        dcat:Resource ;
    rdfs:label "Division D55"@en-AU ;
    rdfs:comment "Division 1 APreliminary - GraphNodeID: D55"@en-AU ;
    skos:broader C1901A00006:56,
        C1901A00006:57,
        C1901A00006:58,
        C1901A00006:59 ;
    skos:definition "Division 1 APreliminary"@en-AU ;
    skos:narrower C1901A00006:54 ;
    skos:prefLabel "Division D55"@en-AU ;
    dcat:accessURL "https://www.legislation.gov.au/C1901A00006/2024-07-01/2024-07-01/text/original/epub/OEBPS/document_1/document_1.html#_Toc172623029"^^xsd:anyURI .

C1901A00006:60 a legcons:Division,
        skos:Concept,
        dcat:Resource ;
    rdfs:label "Division D60"@en-AU ;
    rdfs:comment "Division 1 Prohibited imports - GraphNodeID: D60"@en-AU ;
    skos:broader C1901A00006:61,
        C1901A00006:62,
        C1901A00006:63,
        C1901A00006:64 ;
    skos:definition "Division 1 Prohibited imports"@en-AU ;
    skos:narrower C1901A00006:54 ;
    skos:prefLabel "Division D60"@en-AU ;
    dcat:accessURL "https://www.legislation.gov.au/C1901A00006/2024-07-01/2024-07-01/text/original/epub/OEBPS/document_1/document_1.html#_Toc172623034"^^xsd:anyURI .

C1901A00006:806 a legcons:Subdivision,
        skos:Concept,
        dcat:Resource ;
    rdfs:label "Subdivision S806"@en-AU ;
    rdfs:comment "Subdivision DGoods produced from non originating materials - GraphNodeID: S806"@en-AU ;
    skos:broader C1901A00006:807,
        C1901A00006:808,
        C1901A00006:809,
        C1901A00006:810 ;
    skos:definition "Subdivision DGoods produced from non originating materials"@en-AU ;
    skos:narrower C1901A00006:798 ;
    skos:prefLabel "Subdivision S806"@en-AU ;
    dcat:accessURL "https://www.legislation.gov.au/C1901A00006/2024-07-01/2024-07-01/text/original/epub/OEBPS/document_2/document_2.html#_Toc172624561"^^xsd:anyURI .

C1901A00006:868 a legcons:Part,
        skos:Concept,
        dcat:Resource ;
    rdfs:label "Part P868"@en-AU ;
    rdfs:comment "Part XAAustralian Trusted Trader Programme - GraphNodeID: P868"@en-AU ;
    skos:broader C1901A00006:869,
        C1901A00006:871,
        C1901A00006:878,
        C1901A00006:880 ;
    skos:definition "Part XAAustralian Trusted Trader Programme"@en-AU ;
    skos:narrower C1901A00006:456 ;
    skos:prefLabel "Part P868"@en-AU ;
    dcat:accessURL "https://www.legislation.gov.au/C1901A00006/2024-07-01/2024-07-01/text/original/epub/OEBPS/document_2/document_2.html#_Toc172624623"^^xsd:anyURI .

C1901A00006:882 a legcons:Part,
        skos:Concept,
        dcat:Resource ;
    rdfs:label "Part P882"@en-AU ;
    rdfs:comment "Part XBControlled trials - GraphNodeID: P882"@en-AU ;
    skos:broader C1901A00006:883,
        C1901A00006:886,
        C1901A00006:889,
        C1901A00006:895 ;
    skos:definition "Part XBControlled trials"@en-AU ;
    skos:narrower C1901A00006:456 ;
    skos:prefLabel "Part P882"@en-AU ;
    dcat:accessURL "https://www.legislation.gov.au/C1901A00006/2024-07-01/2024-07-01/text/original/epub/OEBPS/document_2/document_2.html#_Toc172624637"^^xsd:anyURI .

C1901A00006:955 a legcons:Subdivision,
        skos:Concept,
        dcat:Resource ;
    rdfs:label "Subdivision S955"@en-AU ;
    rdfs:comment "Subdivision APreliminary - GraphNodeID: S955"@en-AU ;
    skos:broader C1901A00006:956,
        C1901A00006:957,
        C1901A00006:958,
        C1901A00006:959 ;
    skos:definition "Subdivision APreliminary"@en-AU ;
    skos:narrower C1901A00006:954 ;
    skos:prefLabel "Subdivision S955"@en-AU ;
    dcat:accessURL "https://www.legislation.gov.au/C1901A00006/2024-07-01/2024-07-01/text/original/epub/OEBPS/document_3/document_3.html#_Toc172626989"^^xsd:anyURI .

C1901A00006:1054 a legcons:Subdivision,
        skos:Concept,
        dcat:Resource ;
    rdfs:label "Subdivision S1054"@en-AU ;
    rdfs:comment "Subdivision GBSurrender of prescribed prohibited imports - GraphNodeID: S1054"@en-AU ;
    skos:broader C1901A00006:1055,
        C1901A00006:1056,
        C1901A00006:1057,
        C1901A00006:1058,
        C1901A00006:1059 ;
    skos:definition "Subdivision GBSurrender of prescribed prohibited imports"@en-AU ;
    skos:narrower C1901A00006:954 ;
    skos:prefLabel "Subdivision S1054"@en-AU ;
    dcat:accessURL "https://www.legislation.gov.au/C1901A00006/2024-07-01/2024-07-01/text/original/epub/OEBPS/document_3/document_3.html#_Toc172627088"^^xsd:anyURI .

C1901A00006:1109 a legcons:Subdivision,
        skos:Concept,
        dcat:Resource ;
    rdfs:label "Subdivision S1109"@en-AU ;
    rdfs:comment "Subdivision KMiscellaneous - GraphNodeID: S1109"@en-AU ;
    skos:broader C1901A00006:1110,
        C1901A00006:1111,
        C1901A00006:1112,
        C1901A00006:1113,
        C1901A00006:1114 ;
    skos:definition "Subdivision KMiscellaneous"@en-AU ;
    skos:narrower C1901A00006:954 ;
    skos:prefLabel "Subdivision S1109"@en-AU ;
    dcat:accessURL "https://www.legislation.gov.au/C1901A00006/2024-07-01/2024-07-01/text/original/epub/OEBPS/document_3/document_3.html#_Toc172627143"^^xsd:anyURI .

C1901A00006:1137 a legcons:Subdivision,
        skos:Concept,
        dcat:Resource ;
    rdfs:label "Subdivision S1137"@en-AU ;
    rdfs:comment "Subdivision CAPrescribed equipment for external searches and internal non medical scans - GraphNodeID: S1137"@en-AU ;
    skos:broader C1901A00006:1138,
        C1901A00006:1139,
        C1901A00006:1140,
        C1901A00006:1141,
        C1901A00006:1142 ;
    skos:definition "Subdivision CAPrescribed equipment for external searches and internal non medical scans"@en-AU ;
    skos:narrower C1901A00006:1115 ;
    skos:prefLabel "Subdivision S1137"@en-AU ;
    dcat:accessURL "https://www.legislation.gov.au/C1901A00006/2024-07-01/2024-07-01/text/original/epub/OEBPS/document_3/document_3.html#_Toc172627171"^^xsd:anyURI .

C1901A00006:1143 a legcons:Subdivision,
        skos:Concept,
        dcat:Resource ;
    rdfs:label "Subdivision S1143"@en-AU ;
    rdfs:comment "Subdivision DDetention generally - GraphNodeID: S1143"@en-AU ;
    skos:broader C1901A00006:1144,
        C1901A00006:1145,
        C1901A00006:1146,
        C1901A00006:1147,
        C1901A00006:1148 ;
    skos:definition "Subdivision DDetention generally"@en-AU ;
    skos:narrower C1901A00006:1115 ;
    skos:prefLabel "Subdivision S1143"@en-AU ;
    dcat:accessURL "https://www.legislation.gov.au/C1901A00006/2024-07-01/2024-07-01/text/original/epub/OEBPS/document_3/document_3.html#_Toc172627177"^^xsd:anyURI .

C1901A00006:1192 a legcons:Part,
        skos:Concept,
        dcat:Resource ;
    rdfs:label "Part P1192"@en-AU ;
    rdfs:comment "Part XIIIPenal Provisions - GraphNodeID: P1192"@en-AU ;
    skos:broader C1901A00006:1193,
        C1901A00006:1201,
        C1901A00006:1231,
        C1901A00006:1253,
        C1901A00006:1261 ;
    skos:definition "Part XIIIPenal Provisions"@en-AU ;
    skos:narrower C1901A00006:952 ;
    skos:prefLabel "Part P1192"@en-AU ;
    dcat:accessURL "https://www.legislation.gov.au/C1901A00006/2024-07-01/2024-07-01/text/original/epub/OEBPS/document_3/document_3.html#_Toc172627226"^^xsd:anyURI .

C1901A00006:121 a legcons:Subdivision,
        skos:Concept,
        dcat:Resource ;
    rdfs:label "Subdivision S121"@en-AU ;
    rdfs:comment "Subdivision APreliminary - GraphNodeID: S121"@en-AU ;
    skos:broader C1901A00006:122,
        C1901A00006:123,
        C1901A00006:124,
        C1901A00006:125,
        C1901A00006:126 ;
    skos:definition "Subdivision APreliminary"@en-AU ;
    skos:narrower C1901A00006:120 ;
    skos:prefLabel "Subdivision S121"@en-AU ;
    dcat:accessURL "https://www.legislation.gov.au/C1901A00006/2024-07-01/2024-07-01/text/original/epub/OEBPS/document_1/document_1.html#_Toc172623095"^^xsd:anyURI .

C1901A00006:1291 a legcons:Part,
        skos:Concept,
        dcat:Resource ;
    rdfs:label "Part P1291"@en-AU ;
    rdfs:comment "Part XVATariff concession orders - GraphNodeID: P1291"@en-AU ;
    skos:broader C1901A00006:1292,
        C1901A00006:1297,
        C1901A00006:1308,
        C1901A00006:1314,
        C1901A00006:1321 ;
    skos:definition "Part XVATariff concession orders"@en-AU ;
    skos:narrower C1901A00006:952 ;
    skos:prefLabel "Part P1291"@en-AU ;
    dcat:accessURL "https://www.legislation.gov.au/C1901A00006/2024-07-01/2024-07-01/text/original/epub/OEBPS/document_3/document_3.html#_Toc172627325"^^xsd:anyURI .

C1901A00006:248 a legcons:Part,
        skos:Concept,
        dcat:Resource ;
    rdfs:label "Part P248"@en-AU ;
    rdfs:comment "Part VAAACargo terminals - GraphNodeID: P248"@en-AU ;
    skos:broader C1901A00006:249,
        C1901A00006:252,
        C1901A00006:265,
        C1901A00006:272,
        C1901A00006:276 ;
    skos:definition "Part VAAACargo terminals"@en-AU ;
    skos:narrower C1901A00006:1 ;
    skos:prefLabel "Part P248"@en-AU ;
    dcat:accessURL "https://www.legislation.gov.au/C1901A00006/2024-07-01/2024-07-01/text/original/epub/OEBPS/document_1/document_1.html#_Toc172623222"^^xsd:anyURI .

C1901A00006:898 a legcons:Part,
        skos:Concept,
        dcat:Resource ;
    rdfs:label "Part P898"@en-AU ;
    rdfs:comment "Part XIAgents and customs brokers - GraphNodeID: P898"@en-AU ;
    skos:broader C1901A00006:899,
        C1901A00006:901,
        C1901A00006:906,
        C1901A00006:926,
        C1901A00006:932 ;
    skos:definition "Part XIAgents and customs brokers"@en-AU ;
    skos:narrower C1901A00006:456 ;
    skos:prefLabel "Part P898"@en-AU ;
    dcat:accessURL "https://www.legislation.gov.au/C1901A00006/2024-07-01/2024-07-01/text/original/epub/OEBPS/document_2/document_2.html#_Toc172624653"^^xsd:anyURI .

C1901A00006:952 a legcons:Volume,
        skos:Concept,
        dcat:Resource ;
    rdfs:label "Volume V952"@en-AU ;
    rdfs:comment "Volume 3 - GraphNodeID: V952"@en-AU ;
    skos:broader C1901A00006:1184,
        C1901A00006:1192,
        C1901A00006:1265,
        C1901A00006:1284,
        C1901A00006:1291,
        C1901A00006:953 ;
    skos:definition "Volume 3"@en-AU ;
    skos:prefLabel "Volume V952"@en-AU ;
    dcat:accessURL "https://www.legislation.gov.au/C1901A00006/2024-07-01/2024-07-01/text/original/epub/OEBPS/document_3/document_3.html"^^xsd:anyURI .

C1901A00006:1115 a legcons:Division,
        skos:Concept,
        dcat:Resource ;
    rdfs:label "Division D1115"@en-AU ;
    rdfs:comment "Division 1 BDetention and search of suspects - GraphNodeID: D1115"@en-AU ;
    skos:broader C1901A00006:1116,
        C1901A00006:1121,
        C1901A00006:1125,
        C1901A00006:1137,
        C1901A00006:1143,
        C1901A00006:1149 ;
    skos:definition "Division 1 BDetention and search of suspects"@en-AU ;
    skos:narrower C1901A00006:953 ;
    skos:prefLabel "Division D1115"@en-AU ;
    dcat:accessURL "https://www.legislation.gov.au/C1901A00006/2024-07-01/2024-07-01/text/original/epub/OEBPS/document_3/document_3.html#_Toc172627149"^^xsd:anyURI .

C1901A00006:113 a legcons:Subdivision,
        skos:Concept,
        dcat:Resource ;
    rdfs:label "Subdivision S113"@en-AU ;
    rdfs:comment "Subdivision ERegistering re mail reporters - GraphNodeID: S113"@en-AU ;
    skos:broader C1901A00006:114,
        C1901A00006:115,
        C1901A00006:116,
        C1901A00006:117,
        C1901A00006:118,
        C1901A00006:119 ;
    skos:definition "Subdivision ERegistering re mail reporters"@en-AU ;
    skos:narrower C1901A00006:74 ;
    skos:prefLabel "Subdivision S113"@en-AU ;
    dcat:accessURL "https://www.legislation.gov.au/C1901A00006/2024-07-01/2024-07-01/text/original/epub/OEBPS/document_1/document_1.html#_Toc172623087"^^xsd:anyURI .

C1901A00006:120 a legcons:Division,
        skos:Concept,
        dcat:Resource ;
    rdfs:label "Division D120"@en-AU ;
    rdfs:comment "Division 4 The entry unshipment landing and examination of goods - GraphNodeID: D120"@en-AU ;
    skos:broader C1901A00006:121,
        C1901A00006:127,
        C1901A00006:131,
        C1901A00006:149,
        C1901A00006:156,
        C1901A00006:163 ;
    skos:definition "Division 4 The entry unshipment landing and examination of goods"@en-AU ;
    skos:narrower C1901A00006:54 ;
    skos:prefLabel "Division D120"@en-AU ;
    dcat:accessURL "https://www.legislation.gov.au/C1901A00006/2024-07-01/2024-07-01/text/original/epub/OEBPS/document_1/document_1.html#_Toc172623094"^^xsd:anyURI .

C1901A00006:1466 a legcons:Subdivision,
        skos:Concept,
        dcat:Resource ;
    rdfs:label "Subdivision S1466"@en-AU ;
    rdfs:comment "Subdivision APreliminary - GraphNodeID: S1466"@en-AU ;
    skos:broader C1901A00006:1467,
        C1901A00006:1468,
        C1901A00006:1469,
        C1901A00006:1470,
        C1901A00006:1471,
        C1901A00006:1472 ;
    skos:definition "Subdivision APreliminary"@en-AU ;
    skos:narrower C1901A00006:1465 ;
    skos:prefLabel "Subdivision S1466"@en-AU ;
    dcat:accessURL "https://www.legislation.gov.au/C1901A00006/2024-07-01/2024-07-01/text/original/epub/OEBPS/document_4/document_4.html#_Toc172628900"^^xsd:anyURI .

C1901A00006:149 a legcons:Subdivision,
        skos:Concept,
        dcat:Resource ;
    rdfs:label "Subdivision S149"@en-AU ;
    rdfs:comment "Subdivision BImport declarations - GraphNodeID: S149"@en-AU ;
    skos:broader C1901A00006:150,
        C1901A00006:151,
        C1901A00006:152,
        C1901A00006:153,
        C1901A00006:154,
        C1901A00006:155 ;
    skos:definition "Subdivision BImport declarations"@en-AU ;
    skos:narrower C1901A00006:120 ;
    skos:prefLabel "Subdivision S149"@en-AU ;
    dcat:accessURL "https://www.legislation.gov.au/C1901A00006/2024-07-01/2024-07-01/text/original/epub/OEBPS/document_1/document_1.html#_Toc172623123"^^xsd:anyURI .

C1901A00006:156 a legcons:Subdivision,
        skos:Concept,
        dcat:Resource ;
    rdfs:label "Subdivision S156"@en-AU ;
    rdfs:comment "Subdivision DWarehouse declarations - GraphNodeID: S156"@en-AU ;
    skos:broader C1901A00006:157,
        C1901A00006:158,
        C1901A00006:159,
        C1901A00006:160,
        C1901A00006:161,
        C1901A00006:162 ;
    skos:definition "Subdivision DWarehouse declarations"@en-AU ;
    skos:narrower C1901A00006:120 ;
    skos:prefLabel "Subdivision S156"@en-AU ;
    dcat:accessURL "https://www.legislation.gov.au/C1901A00006/2024-07-01/2024-07-01/text/original/epub/OEBPS/document_1/document_1.html#_Toc172623130"^^xsd:anyURI .

C1901A00006:54 a legcons:Part,
        skos:Concept,
        dcat:Resource ;
    rdfs:label "Part P54"@en-AU ;
    rdfs:comment "Part IVThe importation of goods - GraphNodeID: P54"@en-AU ;
    skos:broader C1901A00006:120,
        C1901A00006:178,
        C1901A00006:55,
        C1901A00006:60,
        C1901A00006:65,
        C1901A00006:74 ;
    skos:definition "Part IVThe importation of goods"@en-AU ;
    skos:narrower C1901A00006:1 ;
    skos:prefLabel "Part P54"@en-AU ;
    dcat:accessURL "https://www.legislation.gov.au/C1901A00006/2024-07-01/2024-07-01/text/original/epub/OEBPS/document_1/document_1.html#_Toc172623028"^^xsd:anyURI .

C1901A00006:698 a legcons:Division,
        skos:Concept,
        dcat:Resource ;
    rdfs:label "Division D698"@en-AU ;
    rdfs:comment "Division 1 HAIndonesian originating goods - GraphNodeID: D698"@en-AU ;
    skos:broader C1901A00006:699,
        C1901A00006:702,
        C1901A00006:704,
        C1901A00006:706,
        C1901A00006:709,
        C1901A00006:712 ;
    skos:definition "Division 1 HAIndonesian originating goods"@en-AU ;
    skos:narrower C1901A00006:475 ;
    skos:prefLabel "Division D698"@en-AU ;
    dcat:accessURL "https://www.legislation.gov.au/C1901A00006/2024-07-01/2024-07-01/text/original/epub/OEBPS/document_2/document_2.html#_Toc172624453"^^xsd:anyURI .

C1901A00006:714 a legcons:Division,
        skos:Concept,
        dcat:Resource ;
    rdfs:label "Division D714"@en-AU ;
    rdfs:comment "Division 1 JKorean originating goods - GraphNodeID: D714"@en-AU ;
    skos:broader C1901A00006:715,
        C1901A00006:718,
        C1901A00006:720,
        C1901A00006:722,
        C1901A00006:725,
        C1901A00006:727 ;
    skos:definition "Division 1 JKorean originating goods"@en-AU ;
    skos:narrower C1901A00006:475 ;
    skos:prefLabel "Division D714"@en-AU ;
    dcat:accessURL "https://www.legislation.gov.au/C1901A00006/2024-07-01/2024-07-01/text/original/epub/OEBPS/document_2/document_2.html#_Toc172624469"^^xsd:anyURI .

C1901A00006:731 a legcons:Division,
        skos:Concept,
        dcat:Resource ;
    rdfs:label "Division D731"@en-AU ;
    rdfs:comment "Division 1 JAIndian originating goods - GraphNodeID: D731"@en-AU ;
    skos:broader C1901A00006:732,
        C1901A00006:735,
        C1901A00006:737,
        C1901A00006:740,
        C1901A00006:742,
        C1901A00006:744 ;
    skos:definition "Division 1 JAIndian originating goods"@en-AU ;
    skos:narrower C1901A00006:475 ;
    skos:prefLabel "Division D731"@en-AU ;
    dcat:accessURL "https://www.legislation.gov.au/C1901A00006/2024-07-01/2024-07-01/text/original/epub/OEBPS/document_2/document_2.html#_Toc172624486"^^xsd:anyURI .

C1901A00006:746 a legcons:Division,
        skos:Concept,
        dcat:Resource ;
    rdfs:label "Division D746"@en-AU ;
    rdfs:comment "Division 1 KJapanese originating goods - GraphNodeID: D746"@en-AU ;
    skos:broader C1901A00006:747,
        C1901A00006:750,
        C1901A00006:752,
        C1901A00006:754,
        C1901A00006:758,
        C1901A00006:760 ;
    skos:definition "Division 1 KJapanese originating goods"@en-AU ;
    skos:narrower C1901A00006:475 ;
    skos:prefLabel "Division D746"@en-AU ;
    dcat:accessURL "https://www.legislation.gov.au/C1901A00006/2024-07-01/2024-07-01/text/original/epub/OEBPS/document_2/document_2.html#_Toc172624501"^^xsd:anyURI .

C1901A00006:798 a legcons:Division,
        skos:Concept,
        dcat:Resource ;
    rdfs:label "Division D798"@en-AU ;
    rdfs:comment "Division 1 NRegional Comprehensive Economic Partnership RCEP originating goods - GraphNodeID: D798"@en-AU ;
    skos:broader C1901A00006:799,
        C1901A00006:802,
        C1901A00006:804,
        C1901A00006:806,
        C1901A00006:811,
        C1901A00006:813 ;
    skos:definition "Division 1 NRegional Comprehensive Economic Partnership RCEP originating goods"@en-AU ;
    skos:narrower C1901A00006:475 ;
    skos:prefLabel "Division D798"@en-AU ;
    dcat:accessURL "https://www.legislation.gov.au/C1901A00006/2024-07-01/2024-07-01/text/original/epub/OEBPS/document_2/document_2.html#_Toc172624553"^^xsd:anyURI .

C1901A00006:953 a legcons:Part,
        skos:Concept,
        dcat:Resource ;
    rdfs:label "Part P953"@en-AU ;
    rdfs:comment "Part XIIOfficers - GraphNodeID: P953"@en-AU ;
    skos:broader C1901A00006:1115,
        C1901A00006:1154,
        C1901A00006:1170,
        C1901A00006:1173,
        C1901A00006:1182,
        C1901A00006:954 ;
    skos:definition "Part XIIOfficers"@en-AU ;
    skos:narrower C1901A00006:952 ;
    skos:prefLabel "Part P953"@en-AU ;
    dcat:accessURL "https://www.legislation.gov.au/C1901A00006/2024-07-01/2024-07-01/text/original/epub/OEBPS/document_3/document_3.html#_Toc172626987"^^xsd:anyURI .

C1901A00006:1072 a legcons:Subdivision,
        skos:Concept,
        dcat:Resource ;
    rdfs:label "Subdivision S1072"@en-AU ;
    rdfs:comment "Subdivision HArrest and related matters - GraphNodeID: S1072"@en-AU ;
    skos:broader C1901A00006:1073,
        C1901A00006:1074,
        C1901A00006:1075,
        C1901A00006:1076,
        C1901A00006:1077,
        C1901A00006:1078,
        C1901A00006:1079 ;
    skos:definition "Subdivision HArrest and related matters"@en-AU ;
    skos:narrower C1901A00006:954 ;
    skos:prefLabel "Subdivision S1072"@en-AU ;
    dcat:accessURL "https://www.legislation.gov.au/C1901A00006/2024-07-01/2024-07-01/text/original/epub/OEBPS/document_3/document_3.html#_Toc172627106"^^xsd:anyURI .

C1901A00006:1329 a legcons:Division,
        skos:Concept,
        dcat:Resource ;
    rdfs:label "Division D1329"@en-AU ;
    rdfs:comment "Division 1 AAnti Dumping Commission and Commissioner - GraphNodeID: D1329"@en-AU ;
    skos:broader C1901A00006:1330,
        C1901A00006:1332,
        C1901A00006:1337,
        C1901A00006:1348,
        C1901A00006:1350,
        C1901A00006:1352,
        C1901A00006:1354 ;
    skos:definition "Division 1 AAnti Dumping Commission and Commissioner"@en-AU ;
    skos:narrower C1901A00006:1327 ;
    skos:prefLabel "Division D1329"@en-AU ;
    dcat:accessURL "https://www.legislation.gov.au/C1901A00006/2024-07-01/2024-07-01/text/original/epub/OEBPS/document_4/document_4.html#_Toc172628763"^^xsd:anyURI .

C1901A00006:456 a legcons:Volume,
        skos:Concept,
        dcat:Resource ;
    rdfs:label "Volume V456"@en-AU ;
    rdfs:comment "Volume 2 - GraphNodeID: V456"@en-AU ;
    skos:broader C1901A00006:457,
        C1901A00006:467,
        C1901A00006:475,
        C1901A00006:864,
        C1901A00006:866,
        C1901A00006:868,
        C1901A00006:882,
        C1901A00006:898 ;
    skos:definition "Volume 2"@en-AU ;
    skos:prefLabel "Volume V456"@en-AU ;
    dcat:accessURL "https://www.legislation.gov.au/C1901A00006/2024-07-01/2024-07-01/text/original/epub/OEBPS/document_2/document_2.html"^^xsd:anyURI .

C1901A00006:520 a legcons:Division,
        skos:Concept,
        dcat:Resource ;
    rdfs:label "Division D520"@en-AU ;
    rdfs:comment "Division 1 BASingaporean originating goods - GraphNodeID: D520"@en-AU ;
    skos:broader C1901A00006:521,
        C1901A00006:524,
        C1901A00006:526,
        C1901A00006:528,
        C1901A00006:531,
        C1901A00006:533,
        C1901A00006:535 ;
    skos:definition "Division 1 BASingaporean originating goods"@en-AU ;
    skos:narrower C1901A00006:475 ;
    skos:prefLabel "Division D520"@en-AU ;
    dcat:accessURL "https://www.legislation.gov.au/C1901A00006/2024-07-01/2024-07-01/text/original/epub/OEBPS/document_2/document_2.html#_Toc172624275"^^xsd:anyURI .

C1901A00006:555 a legcons:Division,
        skos:Concept,
        dcat:Resource ;
    rdfs:label "Division D555"@en-AU ;
    rdfs:comment "Division 1 DThai originating goods - GraphNodeID: D555"@en-AU ;
    skos:broader C1901A00006:556,
        C1901A00006:559,
        C1901A00006:561,
        C1901A00006:563,
        C1901A00006:565,
        C1901A00006:567,
        C1901A00006:569 ;
    skos:definition "Division 1 DThai originating goods"@en-AU ;
    skos:narrower C1901A00006:475 ;
    skos:prefLabel "Division D555"@en-AU ;
    dcat:accessURL "https://www.legislation.gov.au/C1901A00006/2024-07-01/2024-07-01/text/original/epub/OEBPS/document_2/document_2.html#_Toc172624310"^^xsd:anyURI .

C1901A00006:592 a legcons:Division,
        skos:Concept,
        dcat:Resource ;
    rdfs:label "Division D592"@en-AU ;
    rdfs:comment "Division 1 EAPeruvian originating goods - GraphNodeID: D592"@en-AU ;
    skos:broader C1901A00006:593,
        C1901A00006:596,
        C1901A00006:598,
        C1901A00006:600,
        C1901A00006:603,
        C1901A00006:605,
        C1901A00006:607 ;
    skos:definition "Division 1 EAPeruvian originating goods"@en-AU ;
    skos:narrower C1901A00006:475 ;
    skos:prefLabel "Division D592"@en-AU ;
    dcat:accessURL "https://www.legislation.gov.au/C1901A00006/2024-07-01/2024-07-01/text/original/epub/OEBPS/document_2/document_2.html#_Toc172624347"^^xsd:anyURI .

C1901A00006:628 a legcons:Division,
        skos:Concept,
        dcat:Resource ;
    rdfs:label "Division D628"@en-AU ;
    rdfs:comment "Division 1 GASEAN Australia New Zealand AANZ originating goods - GraphNodeID: D628"@en-AU ;
    skos:broader C1901A00006:629,
        C1901A00006:632,
        C1901A00006:634,
        C1901A00006:636,
        C1901A00006:640,
        C1901A00006:642,
        C1901A00006:644 ;
    skos:definition "Division 1 GASEAN Australia New Zealand AANZ originating goods"@en-AU ;
    skos:narrower C1901A00006:475 ;
    skos:prefLabel "Division D628"@en-AU ;
    dcat:accessURL "https://www.legislation.gov.au/C1901A00006/2024-07-01/2024-07-01/text/original/epub/OEBPS/document_2/document_2.html#_Toc172624383"^^xsd:anyURI .

C1901A00006:646 a legcons:Division,
        skos:Concept,
        dcat:Resource ;
    rdfs:label "Division D646"@en-AU ;
    rdfs:comment "Division 1 GAPacific Islands originating goods - GraphNodeID: D646"@en-AU ;
    skos:broader C1901A00006:647,
        C1901A00006:650,
        C1901A00006:652,
        C1901A00006:654,
        C1901A00006:657,
        C1901A00006:659,
        C1901A00006:661 ;
    skos:definition "Division 1 GAPacific Islands originating goods"@en-AU ;
    skos:narrower C1901A00006:475 ;
    skos:prefLabel "Division D646"@en-AU ;
    dcat:accessURL "https://www.legislation.gov.au/C1901A00006/2024-07-01/2024-07-01/text/original/epub/OEBPS/document_2/document_2.html#_Toc172624401"^^xsd:anyURI .

C1901A00006:663 a legcons:Division,
        skos:Concept,
        dcat:Resource ;
    rdfs:label "Division D663"@en-AU ;
    rdfs:comment "Division 1 GBTrans Pacific Partnership originating goods - GraphNodeID: D663"@en-AU ;
    skos:broader C1901A00006:664,
        C1901A00006:667,
        C1901A00006:669,
        C1901A00006:671,
        C1901A00006:674,
        C1901A00006:676,
        C1901A00006:678 ;
    skos:definition "Division 1 GBTrans Pacific Partnership originating goods"@en-AU ;
    skos:narrower C1901A00006:475 ;
    skos:prefLabel "Division D663"@en-AU ;
    dcat:accessURL "https://www.legislation.gov.au/C1901A00006/2024-07-01/2024-07-01/text/original/epub/OEBPS/document_2/document_2.html#_Toc172624418"^^xsd:anyURI .

C1901A00006:680 a legcons:Division,
        skos:Concept,
        dcat:Resource ;
    rdfs:label "Division D680"@en-AU ;
    rdfs:comment "Division 1 HMalaysian originating goods - GraphNodeID: D680"@en-AU ;
    skos:broader C1901A00006:681,
        C1901A00006:684,
        C1901A00006:686,
        C1901A00006:688,
        C1901A00006:692,
        C1901A00006:694,
        C1901A00006:696 ;
    skos:definition "Division 1 HMalaysian originating goods"@en-AU ;
    skos:narrower C1901A00006:475 ;
    skos:prefLabel "Division D680"@en-AU ;
    dcat:accessURL "https://www.legislation.gov.au/C1901A00006/2024-07-01/2024-07-01/text/original/epub/OEBPS/document_2/document_2.html#_Toc172624435"^^xsd:anyURI .

C1901A00006:781 a legcons:Division,
        skos:Concept,
        dcat:Resource ;
    rdfs:label "Division D781"@en-AU ;
    rdfs:comment "Division 1 MHong Kong originating goods - GraphNodeID: D781"@en-AU ;
    skos:broader C1901A00006:782,
        C1901A00006:785,
        C1901A00006:787,
        C1901A00006:789,
        C1901A00006:792,
        C1901A00006:794,
        C1901A00006:796 ;
    skos:definition "Division 1 MHong Kong originating goods"@en-AU ;
    skos:narrower C1901A00006:475 ;
    skos:prefLabel "Division D781"@en-AU ;
    dcat:accessURL "https://www.legislation.gov.au/C1901A00006/2024-07-01/2024-07-01/text/original/epub/OEBPS/document_2/document_2.html#_Toc172624536"^^xsd:anyURI .

C1901A00006:815 a legcons:Division,
        skos:Concept,
        dcat:Resource ;
    rdfs:label "Division D815"@en-AU ;
    rdfs:comment "Division 1 PUK originating goods - GraphNodeID: D815"@en-AU ;
    skos:broader C1901A00006:816,
        C1901A00006:819,
        C1901A00006:821,
        C1901A00006:823,
        C1901A00006:826,
        C1901A00006:828,
        C1901A00006:830 ;
    skos:definition "Division 1 PUK originating goods"@en-AU ;
    skos:narrower C1901A00006:475 ;
    skos:prefLabel "Division D815"@en-AU ;
    dcat:accessURL "https://www.legislation.gov.au/C1901A00006/2024-07-01/2024-07-01/text/original/epub/OEBPS/document_2/document_2.html#_Toc172624570"^^xsd:anyURI .

C1901A00006:991 a legcons:Subdivision,
        skos:Concept,
        dcat:Resource ;
    rdfs:label "Subdivision S991"@en-AU ;
    rdfs:comment "Subdivision DSeizure of goods believed to be forfeited goods - GraphNodeID: S991"@en-AU ;
    skos:broader C1901A00006:992,
        C1901A00006:993,
        C1901A00006:994,
        C1901A00006:995,
        C1901A00006:996,
        C1901A00006:997,
        C1901A00006:998 ;
    skos:definition "Subdivision DSeizure of goods believed to be forfeited goods"@en-AU ;
    skos:narrower C1901A00006:954 ;
    skos:prefLabel "Subdivision S991"@en-AU ;
    dcat:accessURL "https://www.legislation.gov.au/C1901A00006/2024-07-01/2024-07-01/text/original/epub/OEBPS/document_3/document_3.html#_Toc172627025"^^xsd:anyURI .

C1901A00006:537 a legcons:Division,
        skos:Concept,
        dcat:Resource ;
    rdfs:label "Division D537"@en-AU ;
    rdfs:comment "Division 1 CUS originating goods - GraphNodeID: D537"@en-AU ;
    skos:broader C1901A00006:538,
        C1901A00006:541,
        C1901A00006:543,
        C1901A00006:545,
        C1901A00006:547,
        C1901A00006:549,
        C1901A00006:551,
        C1901A00006:553 ;
    skos:definition "Division 1 CUS originating goods"@en-AU ;
    skos:narrower C1901A00006:475 ;
    skos:prefLabel "Division D537"@en-AU ;
    dcat:accessURL "https://www.legislation.gov.au/C1901A00006/2024-07-01/2024-07-01/text/original/epub/OEBPS/document_2/document_2.html#_Toc172624292"^^xsd:anyURI .

C1901A00006:609 a legcons:Division,
        skos:Concept,
        dcat:Resource ;
    rdfs:label "Division D609"@en-AU ;
    rdfs:comment "Division 1 FChilean originating goods - GraphNodeID: D609"@en-AU ;
    skos:broader C1901A00006:610,
        C1901A00006:613,
        C1901A00006:615,
        C1901A00006:617,
        C1901A00006:620,
        C1901A00006:622,
        C1901A00006:624,
        C1901A00006:626 ;
    skos:definition "Division 1 FChilean originating goods"@en-AU ;
    skos:narrower C1901A00006:475 ;
    skos:prefLabel "Division D609"@en-AU ;
    dcat:accessURL "https://www.legislation.gov.au/C1901A00006/2024-07-01/2024-07-01/text/original/epub/OEBPS/document_2/document_2.html#_Toc172624364"^^xsd:anyURI .

C1901A00006:65 a legcons:Division,
        skos:Concept,
        dcat:Resource ;
    rdfs:label "Division D65"@en-AU ;
    rdfs:comment "Division 2 The boarding of ships and aircraft - GraphNodeID: D65"@en-AU ;
    skos:broader C1901A00006:66,
        C1901A00006:67,
        C1901A00006:68,
        C1901A00006:69,
        C1901A00006:70,
        C1901A00006:71,
        C1901A00006:72,
        C1901A00006:73 ;
    skos:definition "Division 2 The boarding of ships and aircraft"@en-AU ;
    skos:narrower C1901A00006:54 ;
    skos:prefLabel "Division D65"@en-AU ;
    dcat:accessURL "https://www.legislation.gov.au/C1901A00006/2024-07-01/2024-07-01/text/original/epub/OEBPS/document_1/document_1.html#_Toc172623039"^^xsd:anyURI .

C1901A00006:762 a legcons:Division,
        skos:Concept,
        dcat:Resource ;
    rdfs:label "Division D762"@en-AU ;
    rdfs:comment "Division 1 LChinese originating goods - GraphNodeID: D762"@en-AU ;
    skos:broader C1901A00006:763,
        C1901A00006:766,
        C1901A00006:768,
        C1901A00006:770,
        C1901A00006:773,
        C1901A00006:775,
        C1901A00006:777,
        C1901A00006:779 ;
    skos:definition "Division 1 LChinese originating goods"@en-AU ;
    skos:narrower C1901A00006:475 ;
    skos:prefLabel "Division D762"@en-AU ;
    dcat:accessURL "https://www.legislation.gov.au/C1901A00006/2024-07-01/2024-07-01/text/original/epub/OEBPS/document_2/document_2.html#_Toc172624517"^^xsd:anyURI .

C1901A00006:571 a legcons:Division,
        skos:Concept,
        dcat:Resource ;
    rdfs:label "Division D571"@en-AU ;
    rdfs:comment "Division 1 ENew Zealand originating goods - GraphNodeID: D571"@en-AU ;
    skos:broader C1901A00006:572,
        C1901A00006:575,
        C1901A00006:577,
        C1901A00006:579,
        C1901A00006:582,
        C1901A00006:584,
        C1901A00006:586,
        C1901A00006:588,
        C1901A00006:590 ;
    skos:definition "Division 1 ENew Zealand originating goods"@en-AU ;
    skos:narrower C1901A00006:475 ;
    skos:prefLabel "Division D571"@en-AU ;
    dcat:accessURL "https://www.legislation.gov.au/C1901A00006/2024-07-01/2024-07-01/text/original/epub/OEBPS/document_2/document_2.html#_Toc172624326"^^xsd:anyURI .

C1901A00006:1 a legcons:Volume,
        skos:Concept,
        dcat:Resource ;
    rdfs:label "Volume V1"@en-AU ;
    rdfs:comment "Volume 1 - GraphNodeID: V1"@en-AU ;
    skos:broader C1901A00006:14,
        C1901A00006:185,
        C1901A00006:2,
        C1901A00006:209,
        C1901A00006:248,
        C1901A00006:279,
        C1901A00006:284,
        C1901A00006:289,
        C1901A00006:305,
        C1901A00006:33,
        C1901A00006:54 ;
    skos:definition "Volume 1"@en-AU ;
    skos:prefLabel "Volume V1"@en-AU ;
    dcat:accessURL "https://www.legislation.gov.au/C1901A00006/2024-07-01/2024-07-01/text/original/epub/OEBPS/document_1/document_1.html"^^xsd:anyURI .

C1901A00006:1337 a legcons:Subdivision,
        skos:Concept,
        dcat:Resource ;
    rdfs:label "Subdivision S1337"@en-AU ;
    rdfs:comment "Subdivision CCommissioner - GraphNodeID: S1337"@en-AU ;
    skos:broader C1901A00006:1338,
        C1901A00006:1339,
        C1901A00006:1340,
        C1901A00006:1341,
        C1901A00006:1342,
        C1901A00006:1343,
        C1901A00006:1344,
        C1901A00006:1345,
        C1901A00006:1346,
        C1901A00006:1347 ;
    skos:definition "Subdivision CCommissioner"@en-AU ;
    skos:narrower C1901A00006:1329 ;
    skos:prefLabel "Subdivision S1337"@en-AU ;
    dcat:accessURL "https://www.legislation.gov.au/C1901A00006/2024-07-01/2024-07-01/text/original/epub/OEBPS/document_4/document_4.html#_Toc172628771"^^xsd:anyURI .

C1901A00006:1042 a legcons:Subdivision,
        skos:Concept,
        dcat:Resource ;
    rdfs:label "Subdivision S1042"@en-AU ;
    rdfs:comment "Subdivision GADealing with goods in transit seized under a section 203 DA warrant - GraphNodeID: S1042"@en-AU ;
    skos:broader C1901A00006:1043,
        C1901A00006:1044,
        C1901A00006:1045,
        C1901A00006:1046,
        C1901A00006:1047,
        C1901A00006:1048,
        C1901A00006:1049,
        C1901A00006:1050,
        C1901A00006:1051,
        C1901A00006:1052,
        C1901A00006:1053 ;
    skos:definition "Subdivision GADealing with goods in transit seized under a section 203 DA warrant"@en-AU ;
    skos:narrower C1901A00006:954 ;
    skos:prefLabel "Subdivision S1042"@en-AU ;
    dcat:accessURL "https://www.legislation.gov.au/C1901A00006/2024-07-01/2024-07-01/text/original/epub/OEBPS/document_3/document_3.html#_Toc172627076"^^xsd:anyURI .

C1901A00006:1060 a legcons:Subdivision,
        skos:Concept,
        dcat:Resource ;
    rdfs:label "Subdivision S1060"@en-AU ;
    rdfs:comment "Subdivision GCPost importation permission - GraphNodeID: S1060"@en-AU ;
    skos:broader C1901A00006:1061,
        C1901A00006:1062,
        C1901A00006:1063,
        C1901A00006:1064,
        C1901A00006:1065,
        C1901A00006:1066,
        C1901A00006:1067,
        C1901A00006:1068,
        C1901A00006:1069,
        C1901A00006:1070,
        C1901A00006:1071 ;
    skos:definition "Subdivision GCPost importation permission"@en-AU ;
    skos:narrower C1901A00006:954 ;
    skos:prefLabel "Subdivision S1060"@en-AU ;
    dcat:accessURL "https://www.legislation.gov.au/C1901A00006/2024-07-01/2024-07-01/text/original/epub/OEBPS/document_3/document_3.html#_Toc172627094"^^xsd:anyURI .

C1901A00006:1125 a legcons:Subdivision,
        skos:Concept,
        dcat:Resource ;
    rdfs:label "Subdivision S1125"@en-AU ;
    rdfs:comment "Subdivision CDetention and internal search of persons suspected of internally concealing substances etc - GraphNodeID: S1125"@en-AU ;
    skos:broader C1901A00006:1126,
        C1901A00006:1127,
        C1901A00006:1128,
        C1901A00006:1129,
        C1901A00006:1130,
        C1901A00006:1131,
        C1901A00006:1132,
        C1901A00006:1133,
        C1901A00006:1134,
        C1901A00006:1135,
        C1901A00006:1136 ;
    skos:definition "Subdivision CDetention and internal search of persons suspected of internally concealing substances etc"@en-AU ;
    skos:narrower C1901A00006:1115 ;
    skos:prefLabel "Subdivision S1125"@en-AU ;
    dcat:accessURL "https://www.legislation.gov.au/C1901A00006/2024-07-01/2024-07-01/text/original/epub/OEBPS/document_3/document_3.html#_Toc172627159"^^xsd:anyURI .

C1901A00006:2 a legcons:Part,
        skos:Concept,
        dcat:Resource ;
    rdfs:label "Part P2"@en-AU ;
    rdfs:comment "Part IIntroductory - GraphNodeID: P2"@en-AU ;
    skos:broader C1901A00006:10,
        C1901A00006:11,
        C1901A00006:12,
        C1901A00006:13,
        C1901A00006:3,
        C1901A00006:4,
        C1901A00006:5,
        C1901A00006:6,
        C1901A00006:7,
        C1901A00006:8,
        C1901A00006:9 ;
    skos:definition "Part IIntroductory"@en-AU ;
    skos:narrower C1901A00006:1 ;
    skos:prefLabel "Part P2"@en-AU ;
    dcat:accessURL "https://www.legislation.gov.au/C1901A00006/2024-07-01/2024-07-01/text/original/epub/OEBPS/document_1/document_1.html#_Toc172622976"^^xsd:anyURI .

C1901A00006:1002 a legcons:Subdivision,
        skos:Concept,
        dcat:Resource ;
    rdfs:label "Subdivision S1002"@en-AU ;
    rdfs:comment "Subdivision EProvisions applicable both to search and seizure warrants - GraphNodeID: S1002"@en-AU ;
    skos:broader C1901A00006:1003,
        C1901A00006:1004,
        C1901A00006:1005,
        C1901A00006:1006,
        C1901A00006:1007,
        C1901A00006:1008,
        C1901A00006:1009,
        C1901A00006:1010,
        C1901A00006:1011,
        C1901A00006:1012,
        C1901A00006:1013,
        C1901A00006:1014 ;
    skos:definition "Subdivision EProvisions applicable both to search and seizure warrants"@en-AU ;
    skos:narrower C1901A00006:954 ;
    skos:prefLabel "Subdivision S1002"@en-AU ;
    dcat:accessURL "https://www.legislation.gov.au/C1901A00006/2024-07-01/2024-07-01/text/original/epub/OEBPS/document_3/document_3.html#_Toc172627036"^^xsd:anyURI .

C1901A00006:1083 a legcons:Subdivision,
        skos:Concept,
        dcat:Resource ;
    rdfs:label "Subdivision S1083"@en-AU ;
    rdfs:comment "Subdivision JGeneral powers to monitor and audit - GraphNodeID: S1083"@en-AU ;
    skos:broader C1901A00006:1084,
        C1901A00006:1085,
        C1901A00006:1086,
        C1901A00006:1087,
        C1901A00006:1088,
        C1901A00006:1089,
        C1901A00006:1090,
        C1901A00006:1091,
        C1901A00006:1092,
        C1901A00006:1093,
        C1901A00006:1094,
        C1901A00006:1095 ;
    skos:definition "Subdivision JGeneral powers to monitor and audit"@en-AU ;
    skos:narrower C1901A00006:954 ;
    skos:prefLabel "Subdivision S1083"@en-AU ;
    dcat:accessURL "https://www.legislation.gov.au/C1901A00006/2024-07-01/2024-07-01/text/original/epub/OEBPS/document_3/document_3.html#_Toc172627117"^^xsd:anyURI .

C1901A00006:1096 a legcons:Subdivision,
        skos:Concept,
        dcat:Resource ;
    rdfs:label "Subdivision S1096"@en-AU ;
    rdfs:comment "Subdivision JAPowers to monitor and auditAustralia United States Free Trade Agreement - GraphNodeID: S1096"@en-AU ;
    skos:broader C1901A00006:1097,
        C1901A00006:1098,
        C1901A00006:1099,
        C1901A00006:1100,
        C1901A00006:1101,
        C1901A00006:1102,
        C1901A00006:1103,
        C1901A00006:1104,
        C1901A00006:1105,
        C1901A00006:1106,
        C1901A00006:1107,
        C1901A00006:1108 ;
    skos:definition "Subdivision JAPowers to monitor and auditAustralia United States Free Trade Agreement"@en-AU ;
    skos:narrower C1901A00006:954 ;
    skos:prefLabel "Subdivision S1096"@en-AU ;
    dcat:accessURL "https://www.legislation.gov.au/C1901A00006/2024-07-01/2024-07-01/text/original/epub/OEBPS/document_3/document_3.html#_Toc172627130"^^xsd:anyURI .

C1901A00006:1327 a legcons:Part,
        skos:Concept,
        dcat:Resource ;
    rdfs:label "Part P1327"@en-AU ;
    rdfs:comment "Part XVBSpecial provisions relating to anti dumping duties - GraphNodeID: P1327"@en-AU ;
    skos:broader C1901A00006:1329,
        C1901A00006:1356,
        C1901A00006:1378,
        C1901A00006:1388,
        C1901A00006:1401,
        C1901A00006:1408,
        C1901A00006:1419,
        C1901A00006:1429,
        C1901A00006:1435,
        C1901A00006:1443,
        C1901A00006:1448,
        C1901A00006:1465 ;
    skos:definition "Part XVBSpecial provisions relating to anti dumping duties"@en-AU ;
    skos:narrower C1901A00006:1326 ;
    skos:prefLabel "Part P1327"@en-AU ;
    dcat:accessURL "https://www.legislation.gov.au/C1901A00006/2024-07-01/2024-07-01/text/original/epub/OEBPS/document_4/document_4.html#_Toc172628761"^^xsd:anyURI .

C1901A00006:978 a legcons:Subdivision,
        skos:Concept,
        dcat:Resource ;
    rdfs:label "Subdivision S978"@en-AU ;
    rdfs:comment "Subdivision CSearch warrants in respect of things believed to be evidential material - GraphNodeID: S978"@en-AU ;
    skos:broader C1901A00006:979,
        C1901A00006:980,
        C1901A00006:981,
        C1901A00006:982,
        C1901A00006:983,
        C1901A00006:984,
        C1901A00006:985,
        C1901A00006:986,
        C1901A00006:987,
        C1901A00006:988,
        C1901A00006:989,
        C1901A00006:990 ;
    skos:definition "Subdivision CSearch warrants in respect of things believed to be evidential material"@en-AU ;
    skos:narrower C1901A00006:954 ;
    skos:prefLabel "Subdivision S978"@en-AU ;
    dcat:accessURL "https://www.legislation.gov.au/C1901A00006/2024-07-01/2024-07-01/text/original/epub/OEBPS/document_3/document_3.html#_Toc172627012"^^xsd:anyURI .

C1901A00006:299 a legcons:Subdivision,
        skos:Concept,
        dcat:Resource ;
    rdfs:label "Subdivision S299"@en-AU ;
    rdfs:comment "Subdivision CHow reports under this Division are to be made - GraphNodeID: S299"@en-AU ;
    skos:broader C1901A00006:300,
        C1901A00006:301,
        C1901A00006:302,
        C1901A00006:304,
        C1901A00006:307,
        C1901A00006:309,
        C1901A00006:310,
        C1901A00006:311,
        C1901A00006:313,
        C1901A00006:314,
        C1901A00006:315,
        C1901A00006:317,
        C1901A00006:318 ;
    skos:definition "Subdivision CHow reports under this Division are to be made"@en-AU ;
    skos:narrower C1901A00006:290 ;
    skos:prefLabel "Subdivision S299"@en-AU ;
    dcat:accessURL "https://www.legislation.gov.au/C1901A00006/2024-07-01/2024-07-01/text/original/epub/OEBPS/document_1/document_1.html#_Toc172623273"^^xsd:anyURI .

C1901A00006:99 a legcons:Subdivision,
        skos:Concept,
        dcat:Resource ;
    rdfs:label "Subdivision S99"@en-AU ;
    rdfs:comment "Subdivision CThe registration rights and obligations of special reporters - GraphNodeID: S99"@en-AU ;
    skos:broader C1901A00006:100,
        C1901A00006:101,
        C1901A00006:102,
        C1901A00006:103,
        C1901A00006:104,
        C1901A00006:105,
        C1901A00006:106,
        C1901A00006:107,
        C1901A00006:108,
        C1901A00006:109,
        C1901A00006:110,
        C1901A00006:111,
        C1901A00006:112 ;
    skos:definition "Subdivision CThe registration rights and obligations of special reporters"@en-AU ;
    skos:narrower C1901A00006:74 ;
    skos:prefLabel "Subdivision S99"@en-AU ;
    dcat:accessURL "https://www.legislation.gov.au/C1901A00006/2024-07-01/2024-07-01/text/original/epub/OEBPS/document_1/document_1.html#_Toc172623073"^^xsd:anyURI .

C1901A00006:1473 a legcons:Subdivision,
        skos:Concept,
        dcat:Resource ;
    rdfs:label "Subdivision S1473"@en-AU ;
    rdfs:comment "Subdivision BReview of Ministerial decisions - GraphNodeID: S1473"@en-AU ;
    skos:broader C1901A00006:1474,
        C1901A00006:1475,
        C1901A00006:1476,
        C1901A00006:1477,
        C1901A00006:1478,
        C1901A00006:1479,
        C1901A00006:1480,
        C1901A00006:1481,
        C1901A00006:1482,
        C1901A00006:1483,
        C1901A00006:1484,
        C1901A00006:1485,
        C1901A00006:1486,
        C1901A00006:1487 ;
    skos:definition "Subdivision BReview of Ministerial decisions"@en-AU ;
    skos:narrower C1901A00006:1465 ;
    skos:prefLabel "Subdivision S1473"@en-AU ;
    dcat:accessURL "https://www.legislation.gov.au/C1901A00006/2024-07-01/2024-07-01/text/original/epub/OEBPS/document_4/document_4.html#_Toc172628907"^^xsd:anyURI .

C1901A00006:1488 a legcons:Subdivision,
        skos:Concept,
        dcat:Resource ;
    rdfs:label "Subdivision S1488"@en-AU ;
    rdfs:comment "Subdivision CReview of Commissioners decisions - GraphNodeID: S1488"@en-AU ;
    skos:broader C1901A00006:1489,
        C1901A00006:1490,
        C1901A00006:1491,
        C1901A00006:1492,
        C1901A00006:1493,
        C1901A00006:1494,
        C1901A00006:1495,
        C1901A00006:1496,
        C1901A00006:1497,
        C1901A00006:1498,
        C1901A00006:1499,
        C1901A00006:1500,
        C1901A00006:1501,
        C1901A00006:1502,
        C1901A00006:1503 ;
    skos:definition "Subdivision CReview of Commissioners decisions"@en-AU ;
    skos:narrower C1901A00006:1465 ;
    skos:prefLabel "Subdivision S1488"@en-AU ;
    dcat:accessURL "https://www.legislation.gov.au/C1901A00006/2024-07-01/2024-07-01/text/original/epub/OEBPS/document_4/document_4.html#_Toc172628922"^^xsd:anyURI .

C1901A00006:954 a legcons:Division,
        skos:Concept,
        dcat:Resource ;
    rdfs:label "Division D954"@en-AU ;
    rdfs:comment "Division 1 Powers of officers - GraphNodeID: D954"@en-AU ;
    skos:broader C1901A00006:1002,
        C1901A00006:1015,
        C1901A00006:1018,
        C1901A00006:1042,
        C1901A00006:1054,
        C1901A00006:1060,
        C1901A00006:1072,
        C1901A00006:1080,
        C1901A00006:1083,
        C1901A00006:1096,
        C1901A00006:1109,
        C1901A00006:955,
        C1901A00006:960,
        C1901A00006:978,
        C1901A00006:991,
        C1901A00006:999 ;
    skos:definition "Division 1 Powers of officers"@en-AU ;
    skos:narrower C1901A00006:953 ;
    skos:prefLabel "Division D954"@en-AU ;
    dcat:accessURL "https://www.legislation.gov.au/C1901A00006/2024-07-01/2024-07-01/text/original/epub/OEBPS/document_3/document_3.html#_Toc172626988"^^xsd:anyURI .

C1901A00006:131 a legcons:Subdivision,
        skos:Concept,
        dcat:Resource ;
    rdfs:label "Subdivision S131"@en-AU ;
    rdfs:comment "Subdivision ABInformation and grant of authority to deal with specified low value goods - GraphNodeID: S131"@en-AU ;
    skos:broader C1901A00006:132,
        C1901A00006:133,
        C1901A00006:134,
        C1901A00006:135,
        C1901A00006:136,
        C1901A00006:137,
        C1901A00006:138,
        C1901A00006:139,
        C1901A00006:140,
        C1901A00006:141,
        C1901A00006:142,
        C1901A00006:143,
        C1901A00006:144,
        C1901A00006:145,
        C1901A00006:146,
        C1901A00006:147,
        C1901A00006:148 ;
    skos:definition "Subdivision ABInformation and grant of authority to deal with specified low value goods"@en-AU ;
    skos:narrower C1901A00006:120 ;
    skos:prefLabel "Subdivision S131"@en-AU ;
    dcat:accessURL "https://www.legislation.gov.au/C1901A00006/2024-07-01/2024-07-01/text/original/epub/OEBPS/document_1/document_1.html#_Toc172623105"^^xsd:anyURI .

C1901A00006:960 a legcons:Subdivision,
        skos:Concept,
        dcat:Resource ;
    rdfs:label "Subdivision S960"@en-AU ;
    rdfs:comment "Subdivision BGeneral regulatory powers - GraphNodeID: S960"@en-AU ;
    skos:broader C1901A00006:961,
        C1901A00006:962,
        C1901A00006:963,
        C1901A00006:964,
        C1901A00006:965,
        C1901A00006:966,
        C1901A00006:967,
        C1901A00006:968,
        C1901A00006:969,
        C1901A00006:970,
        C1901A00006:971,
        C1901A00006:972,
        C1901A00006:973,
        C1901A00006:974,
        C1901A00006:975,
        C1901A00006:976,
        C1901A00006:977 ;
    skos:definition "Subdivision BGeneral regulatory powers"@en-AU ;
    skos:narrower C1901A00006:954 ;
    skos:prefLabel "Subdivision S960"@en-AU ;
    dcat:accessURL "https://www.legislation.gov.au/C1901A00006/2024-07-01/2024-07-01/text/original/epub/OEBPS/document_3/document_3.html#_Toc172626994"^^xsd:anyURI .

C1901A00006:14 a legcons:Part,
        skos:Concept,
        dcat:Resource ;
    rdfs:label "Part P14"@en-AU ;
    rdfs:comment "Part IIAdministration - GraphNodeID: P14"@en-AU ;
    skos:broader C1901A00006:15,
        C1901A00006:16,
        C1901A00006:17,
        C1901A00006:18,
        C1901A00006:19,
        C1901A00006:20,
        C1901A00006:21,
        C1901A00006:22,
        C1901A00006:23,
        C1901A00006:24,
        C1901A00006:25,
        C1901A00006:26,
        C1901A00006:27,
        C1901A00006:28,
        C1901A00006:29,
        C1901A00006:30,
        C1901A00006:31,
        C1901A00006:32 ;
    skos:definition "Part IIAdministration"@en-AU ;
    skos:narrower C1901A00006:1 ;
    skos:prefLabel "Part P14"@en-AU ;
    dcat:accessURL "https://www.legislation.gov.au/C1901A00006/2024-07-01/2024-07-01/text/original/epub/OEBPS/document_1/document_1.html#_Toc172622988"^^xsd:anyURI .

C1901A00006:33 a legcons:Part,
        skos:Concept,
        dcat:Resource ;
    rdfs:label "Part P33"@en-AU ;
    rdfs:comment "Part IIICustoms control examination and securities generally - GraphNodeID: P33"@en-AU ;
    skos:broader C1901A00006:34,
        C1901A00006:35,
        C1901A00006:36,
        C1901A00006:37,
        C1901A00006:38,
        C1901A00006:39,
        C1901A00006:40,
        C1901A00006:41,
        C1901A00006:42,
        C1901A00006:43,
        C1901A00006:44,
        C1901A00006:45,
        C1901A00006:46,
        C1901A00006:47,
        C1901A00006:48,
        C1901A00006:49,
        C1901A00006:50,
        C1901A00006:51,
        C1901A00006:52,
        C1901A00006:53 ;
    skos:definition "Part IIICustoms control examination and securities generally"@en-AU ;
    skos:narrower C1901A00006:1 ;
    skos:prefLabel "Part P33"@en-AU ;
    dcat:accessURL "https://www.legislation.gov.au/C1901A00006/2024-07-01/2024-07-01/text/original/epub/OEBPS/document_1/document_1.html#_Toc172623007"^^xsd:anyURI .

C1901A00006:1018 a legcons:Subdivision,
        skos:Concept,
        dcat:Resource ;
    rdfs:label "Subdivision S1018"@en-AU ;
    rdfs:comment "Subdivision GDealing with goods seized as forfeited goods - GraphNodeID: S1018"@en-AU ;
    skos:broader C1901A00006:1019,
        C1901A00006:1020,
        C1901A00006:1021,
        C1901A00006:1022,
        C1901A00006:1023,
        C1901A00006:1024,
        C1901A00006:1025,
        C1901A00006:1026,
        C1901A00006:1027,
        C1901A00006:1028,
        C1901A00006:1029,
        C1901A00006:1030,
        C1901A00006:1031,
        C1901A00006:1032,
        C1901A00006:1033,
        C1901A00006:1034,
        C1901A00006:1035,
        C1901A00006:1036,
        C1901A00006:1037,
        C1901A00006:1038,
        C1901A00006:1039,
        C1901A00006:1040,
        C1901A00006:1041 ;
    skos:definition "Subdivision GDealing with goods seized as forfeited goods"@en-AU ;
    skos:narrower C1901A00006:954 ;
    skos:prefLabel "Subdivision S1018"@en-AU ;
    dcat:accessURL "https://www.legislation.gov.au/C1901A00006/2024-07-01/2024-07-01/text/original/epub/OEBPS/document_3/document_3.html#_Toc172627052"^^xsd:anyURI .

C1901A00006:75 a legcons:Subdivision,
        skos:Concept,
        dcat:Resource ;
    rdfs:label "Subdivision S75"@en-AU ;
    rdfs:comment "Subdivision AGeneral reporting requirements - GraphNodeID: S75"@en-AU ;
    skos:broader C1901A00006:76,
        C1901A00006:77,
        C1901A00006:78,
        C1901A00006:79,
        C1901A00006:80,
        C1901A00006:81,
        C1901A00006:82,
        C1901A00006:83,
        C1901A00006:84,
        C1901A00006:85,
        C1901A00006:86,
        C1901A00006:87,
        C1901A00006:88,
        C1901A00006:89,
        C1901A00006:90,
        C1901A00006:91,
        C1901A00006:92,
        C1901A00006:93,
        C1901A00006:94,
        C1901A00006:95,
        C1901A00006:96,
        C1901A00006:97,
        C1901A00006:98 ;
    skos:definition "Subdivision AGeneral reporting requirements"@en-AU ;
    skos:narrower C1901A00006:74 ;
    skos:prefLabel "Subdivision S75"@en-AU ;
    dcat:accessURL "https://www.legislation.gov.au/C1901A00006/2024-07-01/2024-07-01/text/original/epub/OEBPS/document_1/document_1.html#_Toc172623049"^^xsd:anyURI .

C1901A00006:475 a legcons:Part,
        skos:Concept,
        dcat:Resource ;
    rdfs:label "Part P475"@en-AU ;
    rdfs:comment "Part VIIIThe duties - GraphNodeID: P475"@en-AU ;
    skos:broader C1901A00006:476,
        C1901A00006:497,
        C1901A00006:502,
        C1901A00006:520,
        C1901A00006:537,
        C1901A00006:555,
        C1901A00006:571,
        C1901A00006:592,
        C1901A00006:609,
        C1901A00006:628,
        C1901A00006:646,
        C1901A00006:663,
        C1901A00006:680,
        C1901A00006:698,
        C1901A00006:714,
        C1901A00006:731,
        C1901A00006:746,
        C1901A00006:762,
        C1901A00006:781,
        C1901A00006:798,
        C1901A00006:815,
        C1901A00006:832,
        C1901A00006:852,
        C1901A00006:862 ;
    skos:definition "Part VIIIThe duties"@en-AU ;
    skos:narrower C1901A00006:456 ;
    skos:prefLabel "Part P475"@en-AU ;
    dcat:accessURL "https://www.legislation.gov.au/C1901A00006/2024-07-01/2024-07-01/text/original/epub/OEBPS/document_2/document_2.html#_Toc172624230"^^xsd:anyURI .

C1901A00006:305 a legcons:Part,
        skos:Concept,
        dcat:Resource ;
    rdfs:label "Part P305"@en-AU ;
    rdfs:comment "Part VIThe exportation of goods - GraphNodeID: P305"@en-AU ;
    skos:broader C1901A00006:306,
        C1901A00006:308,
        C1901A00006:312,
        C1901A00006:316,
        C1901A00006:319,
        C1901A00006:353,
        C1901A00006:365,
        C1901A00006:370,
        C1901A00006:375,
        C1901A00006:377,
        C1901A00006:382,
        C1901A00006:387,
        C1901A00006:392,
        C1901A00006:397,
        C1901A00006:402,
        C1901A00006:407,
        C1901A00006:412,
        C1901A00006:417,
        C1901A00006:422,
        C1901A00006:427,
        C1901A00006:432,
        C1901A00006:437,
        C1901A00006:442,
        C1901A00006:447,
        C1901A00006:452 ;
    skos:definition "Part VIThe exportation of goods"@en-AU ;
    skos:narrower C1901A00006:1 ;
    skos:prefLabel "Part P305"@en-AU ;
    dcat:accessURL "https://www.legislation.gov.au/C1901A00006/2024-07-01/2024-07-01/text/original/epub/OEBPS/document_1/document_1.html#_Toc172623279"^^xsd:anyURI .

C1901A00006:830 a legcons:Subdivision,
        skos:Concept,
        dcat:Resource ;
    rdfs:label "Subdivision S830"@en-AU ;
    rdfs:comment "Subdivision GRegulations - GraphNodeID: S830"@en-AU ;
    skos:broader C1901A00006:831,
        C1901A00006:833,
        C1901A00006:834,
        C1901A00006:835,
        C1901A00006:836,
        C1901A00006:837,
        C1901A00006:838,
        C1901A00006:839,
        C1901A00006:840,
        C1901A00006:841,
        C1901A00006:842,
        C1901A00006:843,
        C1901A00006:844,
        C1901A00006:845,
        C1901A00006:846,
        C1901A00006:847,
        C1901A00006:848,
        C1901A00006:849,
        C1901A00006:850,
        C1901A00006:851,
        C1901A00006:853,
        C1901A00006:854,
        C1901A00006:855,
        C1901A00006:856,
        C1901A00006:857,
        C1901A00006:858,
        C1901A00006:859,
        C1901A00006:860,
        C1901A00006:861,
        C1901A00006:863,
        C1901A00006:865,
        C1901A00006:867,
        C1901A00006:870 ;
    skos:definition "Subdivision GRegulations"@en-AU ;
    skos:narrower C1901A00006:815 ;
    skos:prefLabel "Subdivision S830"@en-AU ;
    dcat:accessURL "https://www.legislation.gov.au/C1901A00006/2024-07-01/2024-07-01/text/original/epub/OEBPS/document_2/document_2.html#_Toc172624585"^^xsd:anyURI .

C1901A00006:1504 a legcons:Subdivision,
        skos:Concept,
        dcat:Resource ;
    rdfs:label "Subdivision S1504"@en-AU ;
    rdfs:comment "Subdivision DPublic record in relation to reviews - GraphNodeID: S1504"@en-AU ;
    skos:broader C1901A00006:1505,
        C1901A00006:1506,
        C1901A00006:1507,
        C1901A00006:1509,
        C1901A00006:1510,
        C1901A00006:1511,
        C1901A00006:1512,
        C1901A00006:1513,
        C1901A00006:1514,
        C1901A00006:1515,
        C1901A00006:1516,
        C1901A00006:1518,
        C1901A00006:1519,
        C1901A00006:1520,
        C1901A00006:1521,
        C1901A00006:1522,
        C1901A00006:1523,
        C1901A00006:1524,
        C1901A00006:1525,
        C1901A00006:1526,
        C1901A00006:1527,
        C1901A00006:1529,
        C1901A00006:1530,
        C1901A00006:1531,
        C1901A00006:1532,
        C1901A00006:1533,
        C1901A00006:1534,
        C1901A00006:1535,
        C1901A00006:1536,
        C1901A00006:1537,
        C1901A00006:1538,
        C1901A00006:1539,
        C1901A00006:1540,
        C1901A00006:1541,
        C1901A00006:1542,
        C1901A00006:1543,
        C1901A00006:1544,
        C1901A00006:1547,
        C1901A00006:1548,
        C1901A00006:1549,
        C1901A00006:1550,
        C1901A00006:1551 ;
    skos:definition "Subdivision DPublic record in relation to reviews"@en-AU ;
    skos:narrower C1901A00006:1465 ;
    skos:prefLabel "Subdivision S1504"@en-AU ;
    dcat:accessURL "https://www.legislation.gov.au/C1901A00006/2024-07-01/2024-07-01/text/original/epub/OEBPS/document_4/document_4.html#_Toc172628938"^^xsd:anyURI .

C1901A00006:875 a legcons:Subdivision,
        skos:Concept,
        dcat:Resource ;
    rdfs:label "Subdivision S875"@en-AU ;
    rdfs:comment "Subdivision CGeneral provisions relating to trusted trader agreements - GraphNodeID: S875"@en-AU ;
    skos:broader C1901A00006:876,
        C1901A00006:877,
        C1901A00006:879,
        C1901A00006:881,
        C1901A00006:884,
        C1901A00006:885,
        C1901A00006:887,
        C1901A00006:888,
        C1901A00006:890,
        C1901A00006:891,
        C1901A00006:892,
        C1901A00006:893,
        C1901A00006:894,
        C1901A00006:896,
        C1901A00006:897,
        C1901A00006:900,
        C1901A00006:902,
        C1901A00006:903,
        C1901A00006:904,
        C1901A00006:905,
        C1901A00006:907,
        C1901A00006:908,
        C1901A00006:909,
        C1901A00006:910,
        C1901A00006:911,
        C1901A00006:912,
        C1901A00006:913,
        C1901A00006:914,
        C1901A00006:915,
        C1901A00006:916,
        C1901A00006:917,
        C1901A00006:918,
        C1901A00006:919,
        C1901A00006:920,
        C1901A00006:921,
        C1901A00006:922,
        C1901A00006:923,
        C1901A00006:924,
        C1901A00006:925,
        C1901A00006:927,
        C1901A00006:928,
        C1901A00006:929,
        C1901A00006:930,
        C1901A00006:931,
        C1901A00006:933,
        C1901A00006:934,
        C1901A00006:935,
        C1901A00006:936,
        C1901A00006:937,
        C1901A00006:938,
        C1901A00006:939,
        C1901A00006:940,
        C1901A00006:941,
        C1901A00006:942,
        C1901A00006:943,
        C1901A00006:944,
        C1901A00006:945,
        C1901A00006:946,
        C1901A00006:947,
        C1901A00006:948,
        C1901A00006:949,
        C1901A00006:950,
        C1901A00006:951 ;
    skos:definition "Subdivision CGeneral provisions relating to trusted trader agreements"@en-AU ;
    skos:narrower C1901A00006:871 ;
    skos:prefLabel "Subdivision S875"@en-AU ;
    dcat:accessURL "https://www.legislation.gov.au/C1901A00006/2024-07-01/2024-07-01/text/original/epub/OEBPS/document_2/document_2.html#_Toc172624630"^^xsd:anyURI .

C1901A00006:1354 a legcons:Subdivision,
        skos:Concept,
        dcat:Resource ;
    rdfs:label "Subdivision S1354"@en-AU ;
    rdfs:comment "Subdivision GDisclosure of information - GraphNodeID: S1354"@en-AU ;
    skos:broader C1901A00006:1355,
        C1901A00006:1357,
        C1901A00006:1358,
        C1901A00006:1359,
        C1901A00006:1360,
        C1901A00006:1361,
        C1901A00006:1362,
        C1901A00006:1363,
        C1901A00006:1364,
        C1901A00006:1365,
        C1901A00006:1366,
        C1901A00006:1367,
        C1901A00006:1368,
        C1901A00006:1369,
        C1901A00006:1370,
        C1901A00006:1371,
        C1901A00006:1372,
        C1901A00006:1373,
        C1901A00006:1374,
        C1901A00006:1375,
        C1901A00006:1376,
        C1901A00006:1377,
        C1901A00006:1379,
        C1901A00006:1380,
        C1901A00006:1381,
        C1901A00006:1382,
        C1901A00006:1383,
        C1901A00006:1384,
        C1901A00006:1385,
        C1901A00006:1386,
        C1901A00006:1387,
        C1901A00006:1389,
        C1901A00006:1390,
        C1901A00006:1391,
        C1901A00006:1392,
        C1901A00006:1393,
        C1901A00006:1394,
        C1901A00006:1395,
        C1901A00006:1396,
        C1901A00006:1397,
        C1901A00006:1398,
        C1901A00006:1399,
        C1901A00006:1400,
        C1901A00006:1402,
        C1901A00006:1403,
        C1901A00006:1404,
        C1901A00006:1405,
        C1901A00006:1406,
        C1901A00006:1407,
        C1901A00006:1409,
        C1901A00006:1410,
        C1901A00006:1411,
        C1901A00006:1412,
        C1901A00006:1413,
        C1901A00006:1414,
        C1901A00006:1415,
        C1901A00006:1416,
        C1901A00006:1417,
        C1901A00006:1418,
        C1901A00006:1420,
        C1901A00006:1421,
        C1901A00006:1422,
        C1901A00006:1423,
        C1901A00006:1424,
        C1901A00006:1425,
        C1901A00006:1426,
        C1901A00006:1427,
        C1901A00006:1428,
        C1901A00006:1430,
        C1901A00006:1431,
        C1901A00006:1432,
        C1901A00006:1433,
        C1901A00006:1434,
        C1901A00006:1436,
        C1901A00006:1437,
        C1901A00006:1438,
        C1901A00006:1439,
        C1901A00006:1440,
        C1901A00006:1441,
        C1901A00006:1442,
        C1901A00006:1444,
        C1901A00006:1445,
        C1901A00006:1446,
        C1901A00006:1447,
        C1901A00006:1449,
        C1901A00006:1450,
        C1901A00006:1451,
        C1901A00006:1452,
        C1901A00006:1453,
        C1901A00006:1454,
        C1901A00006:1455,
        C1901A00006:1456,
        C1901A00006:1457,
        C1901A00006:1458,
        C1901A00006:1459,
        C1901A00006:1460,
        C1901A00006:1461,
        C1901A00006:1462,
        C1901A00006:1463,
        C1901A00006:1464 ;
    skos:definition "Subdivision GDisclosure of information"@en-AU ;
    skos:narrower C1901A00006:1329 ;
    skos:prefLabel "Subdivision S1354"@en-AU ;
    dcat:accessURL "https://www.legislation.gov.au/C1901A00006/2024-07-01/2024-07-01/text/original/epub/OEBPS/document_4/document_4.html#_Toc172628788"^^xsd:anyURI .

C1901A00006:163 a legcons:Subdivision,
        skos:Concept,
        dcat:Resource ;
    rdfs:label "Subdivision S163"@en-AU ;
    rdfs:comment "Subdivision EGeneral - GraphNodeID: S163"@en-AU ;
    skos:broader C1901A00006:164,
        C1901A00006:165,
        C1901A00006:166,
        C1901A00006:167,
        C1901A00006:168,
        C1901A00006:169,
        C1901A00006:170,
        C1901A00006:171,
        C1901A00006:172,
        C1901A00006:173,
        C1901A00006:174,
        C1901A00006:175,
        C1901A00006:176,
        C1901A00006:177,
        C1901A00006:179,
        C1901A00006:180,
        C1901A00006:181,
        C1901A00006:182,
        C1901A00006:183,
        C1901A00006:184,
        C1901A00006:186,
        C1901A00006:187,
        C1901A00006:188,
        C1901A00006:189,
        C1901A00006:190,
        C1901A00006:191,
        C1901A00006:192,
        C1901A00006:193,
        C1901A00006:194,
        C1901A00006:195,
        C1901A00006:196,
        C1901A00006:197,
        C1901A00006:198,
        C1901A00006:199,
        C1901A00006:200,
        C1901A00006:201,
        C1901A00006:202,
        C1901A00006:203,
        C1901A00006:204,
        C1901A00006:205,
        C1901A00006:206,
        C1901A00006:207,
        C1901A00006:208,
        C1901A00006:210,
        C1901A00006:211,
        C1901A00006:212,
        C1901A00006:213,
        C1901A00006:214,
        C1901A00006:215,
        C1901A00006:216,
        C1901A00006:217,
        C1901A00006:218,
        C1901A00006:219,
        C1901A00006:220,
        C1901A00006:221,
        C1901A00006:222,
        C1901A00006:223,
        C1901A00006:224,
        C1901A00006:225,
        C1901A00006:226,
        C1901A00006:227,
        C1901A00006:228,
        C1901A00006:229,
        C1901A00006:230,
        C1901A00006:231,
        C1901A00006:232,
        C1901A00006:233,
        C1901A00006:234,
        C1901A00006:235,
        C1901A00006:236,
        C1901A00006:237,
        C1901A00006:238,
        C1901A00006:239,
        C1901A00006:240,
        C1901A00006:241,
        C1901A00006:242,
        C1901A00006:243,
        C1901A00006:244,
        C1901A00006:245,
        C1901A00006:246,
        C1901A00006:247,
        C1901A00006:250,
        C1901A00006:251,
        C1901A00006:253,
        C1901A00006:254,
        C1901A00006:255,
        C1901A00006:256,
        C1901A00006:257,
        C1901A00006:258,
        C1901A00006:259,
        C1901A00006:260,
        C1901A00006:261,
        C1901A00006:262,
        C1901A00006:263,
        C1901A00006:264,
        C1901A00006:266,
        C1901A00006:267,
        C1901A00006:268,
        C1901A00006:269,
        C1901A00006:270,
        C1901A00006:271,
        C1901A00006:273,
        C1901A00006:274,
        C1901A00006:275,
        C1901A00006:277,
        C1901A00006:278,
        C1901A00006:280,
        C1901A00006:281,
        C1901A00006:282,
        C1901A00006:283,
        C1901A00006:285,
        C1901A00006:286,
        C1901A00006:287,
        C1901A00006:288 ;
    skos:definition "Subdivision EGeneral"@en-AU ;
    skos:narrower C1901A00006:120 ;
    skos:prefLabel "Subdivision S163"@en-AU ;
    dcat:accessURL "https://www.legislation.gov.au/C1901A00006/2024-07-01/2024-07-01/text/original/epub/OEBPS/document_1/document_1.html#_Toc172623137"^^xsd:anyURI .

C1901A00006:1162 a legcons:Subdivision,
        skos:Concept,
        dcat:Resource ;
    rdfs:label "Subdivision S1162"@en-AU ;
    rdfs:comment "Subdivision CMatters affecting detention generally - GraphNodeID: S1162"@en-AU ;
    skos:broader C1901A00006:1163,
        C1901A00006:1164,
        C1901A00006:1165,
        C1901A00006:1166,
        C1901A00006:1167,
        C1901A00006:1168,
        C1901A00006:1169,
        C1901A00006:1171,
        C1901A00006:1172,
        C1901A00006:1174,
        C1901A00006:1175,
        C1901A00006:1176,
        C1901A00006:1177,
        C1901A00006:1178,
        C1901A00006:1179,
        C1901A00006:1180,
        C1901A00006:1181,
        C1901A00006:1183,
        C1901A00006:1185,
        C1901A00006:1186,
        C1901A00006:1187,
        C1901A00006:1188,
        C1901A00006:1189,
        C1901A00006:1190,
        C1901A00006:1191,
        C1901A00006:1194,
        C1901A00006:1195,
        C1901A00006:1196,
        C1901A00006:1197,
        C1901A00006:1198,
        C1901A00006:1199,
        C1901A00006:1200,
        C1901A00006:1202,
        C1901A00006:1203,
        C1901A00006:1204,
        C1901A00006:1205,
        C1901A00006:1206,
        C1901A00006:1207,
        C1901A00006:1208,
        C1901A00006:1209,
        C1901A00006:1210,
        C1901A00006:1211,
        C1901A00006:1212,
        C1901A00006:1213,
        C1901A00006:1214,
        C1901A00006:1215,
        C1901A00006:1216,
        C1901A00006:1217,
        C1901A00006:1218,
        C1901A00006:1219,
        C1901A00006:1220,
        C1901A00006:1221,
        C1901A00006:1222,
        C1901A00006:1223,
        C1901A00006:1224,
        C1901A00006:1225,
        C1901A00006:1226,
        C1901A00006:1227,
        C1901A00006:1228,
        C1901A00006:1229,
        C1901A00006:1230,
        C1901A00006:1232,
        C1901A00006:1233,
        C1901A00006:1234,
        C1901A00006:1235,
        C1901A00006:1236,
        C1901A00006:1237,
        C1901A00006:1238,
        C1901A00006:1239,
        C1901A00006:1240,
        C1901A00006:1241,
        C1901A00006:1242,
        C1901A00006:1243,
        C1901A00006:1244,
        C1901A00006:1245,
        C1901A00006:1246,
        C1901A00006:1247,
        C1901A00006:1248,
        C1901A00006:1249,
        C1901A00006:1250,
        C1901A00006:1251,
        C1901A00006:1252,
        C1901A00006:1254,
        C1901A00006:1255,
        C1901A00006:1256,
        C1901A00006:1257,
        C1901A00006:1258,
        C1901A00006:1259,
        C1901A00006:1260,
        C1901A00006:1262,
        C1901A00006:1263,
        C1901A00006:1264,
        C1901A00006:1266,
        C1901A00006:1267,
        C1901A00006:1268,
        C1901A00006:1269,
        C1901A00006:1270,
        C1901A00006:1271,
        C1901A00006:1272,
        C1901A00006:1273,
        C1901A00006:1274,
        C1901A00006:1275,
        C1901A00006:1276,
        C1901A00006:1277,
        C1901A00006:1278,
        C1901A00006:1279,
        C1901A00006:1280,
        C1901A00006:1281,
        C1901A00006:1282,
        C1901A00006:1283,
        C1901A00006:1285,
        C1901A00006:1286,
        C1901A00006:1287,
        C1901A00006:1288,
        C1901A00006:1289,
        C1901A00006:1290,
        C1901A00006:1293,
        C1901A00006:1294,
        C1901A00006:1295,
        C1901A00006:1296,
        C1901A00006:1298,
        C1901A00006:1299,
        C1901A00006:1300,
        C1901A00006:1301,
        C1901A00006:1302,
        C1901A00006:1303,
        C1901A00006:1304,
        C1901A00006:1305,
        C1901A00006:1306,
        C1901A00006:1307,
        C1901A00006:1309,
        C1901A00006:1310,
        C1901A00006:1311,
        C1901A00006:1312,
        C1901A00006:1313,
        C1901A00006:1315,
        C1901A00006:1316,
        C1901A00006:1317,
        C1901A00006:1318,
        C1901A00006:1319,
        C1901A00006:1320,
        C1901A00006:1322,
        C1901A00006:1323,
        C1901A00006:1324,
        C1901A00006:1325,
        C1901A00006:1328 ;
    skos:definition "Subdivision CMatters affecting detention generally"@en-AU ;
    skos:narrower C1901A00006:1154 ;
    skos:prefLabel "Subdivision S1162"@en-AU ;
    dcat:accessURL "https://www.legislation.gov.au/C1901A00006/2024-07-01/2024-07-01/text/original/epub/OEBPS/document_3/document_3.html#_Toc172627196"^^xsd:anyURI .

C1901A00006:327 a legcons:Subdivision,
        skos:Concept,
        dcat:Resource ;
    rdfs:label "Subdivision S327"@en-AU ;
    rdfs:comment "Subdivision DGeneral - GraphNodeID: S327"@en-AU ;
    skos:broader C1901A00006:328,
        C1901A00006:329,
        C1901A00006:330,
        C1901A00006:331,
        C1901A00006:332,
        C1901A00006:333,
        C1901A00006:334,
        C1901A00006:335,
        C1901A00006:336,
        C1901A00006:337,
        C1901A00006:338,
        C1901A00006:339,
        C1901A00006:340,
        C1901A00006:341,
        C1901A00006:342,
        C1901A00006:343,
        C1901A00006:344,
        C1901A00006:345,
        C1901A00006:346,
        C1901A00006:347,
        C1901A00006:348,
        C1901A00006:349,
        C1901A00006:350,
        C1901A00006:351,
        C1901A00006:352,
        C1901A00006:354,
        C1901A00006:355,
        C1901A00006:356,
        C1901A00006:357,
        C1901A00006:358,
        C1901A00006:359,
        C1901A00006:360,
        C1901A00006:361,
        C1901A00006:362,
        C1901A00006:363,
        C1901A00006:364,
        C1901A00006:366,
        C1901A00006:367,
        C1901A00006:368,
        C1901A00006:369,
        C1901A00006:371,
        C1901A00006:372,
        C1901A00006:373,
        C1901A00006:374,
        C1901A00006:376,
        C1901A00006:378,
        C1901A00006:379,
        C1901A00006:380,
        C1901A00006:381,
        C1901A00006:383,
        C1901A00006:384,
        C1901A00006:385,
        C1901A00006:386,
        C1901A00006:388,
        C1901A00006:389,
        C1901A00006:390,
        C1901A00006:391,
        C1901A00006:393,
        C1901A00006:394,
        C1901A00006:395,
        C1901A00006:396,
        C1901A00006:398,
        C1901A00006:399,
        C1901A00006:400,
        C1901A00006:401,
        C1901A00006:403,
        C1901A00006:404,
        C1901A00006:405,
        C1901A00006:406,
        C1901A00006:408,
        C1901A00006:409,
        C1901A00006:410,
        C1901A00006:411,
        C1901A00006:413,
        C1901A00006:414,
        C1901A00006:415,
        C1901A00006:416,
        C1901A00006:418,
        C1901A00006:419,
        C1901A00006:420,
        C1901A00006:421,
        C1901A00006:423,
        C1901A00006:424,
        C1901A00006:425,
        C1901A00006:426,
        C1901A00006:428,
        C1901A00006:429,
        C1901A00006:430,
        C1901A00006:431,
        C1901A00006:433,
        C1901A00006:434,
        C1901A00006:435,
        C1901A00006:436,
        C1901A00006:438,
        C1901A00006:439,
        C1901A00006:440,
        C1901A00006:441,
        C1901A00006:443,
        C1901A00006:444,
        C1901A00006:445,
        C1901A00006:446,
        C1901A00006:448,
        C1901A00006:449,
        C1901A00006:450,
        C1901A00006:451,
        C1901A00006:453,
        C1901A00006:454,
        C1901A00006:455,
        C1901A00006:458,
        C1901A00006:459,
        C1901A00006:460,
        C1901A00006:461,
        C1901A00006:462,
        C1901A00006:463,
        C1901A00006:464,
        C1901A00006:465,
        C1901A00006:466,
        C1901A00006:468,
        C1901A00006:469,
        C1901A00006:470,
        C1901A00006:471,
        C1901A00006:472,
        C1901A00006:473,
        C1901A00006:474,
        C1901A00006:477,
        C1901A00006:478,
        C1901A00006:479,
        C1901A00006:480,
        C1901A00006:481,
        C1901A00006:482,
        C1901A00006:483,
        C1901A00006:484,
        C1901A00006:485,
        C1901A00006:486,
        C1901A00006:487,
        C1901A00006:488,
        C1901A00006:489,
        C1901A00006:490,
        C1901A00006:491,
        C1901A00006:492,
        C1901A00006:493,
        C1901A00006:494,
        C1901A00006:495,
        C1901A00006:496,
        C1901A00006:498,
        C1901A00006:499,
        C1901A00006:500,
        C1901A00006:501,
        C1901A00006:503,
        C1901A00006:504,
        C1901A00006:505,
        C1901A00006:506,
        C1901A00006:507,
        C1901A00006:508,
        C1901A00006:509,
        C1901A00006:510,
        C1901A00006:511,
        C1901A00006:512,
        C1901A00006:513,
        C1901A00006:514,
        C1901A00006:515,
        C1901A00006:516,
        C1901A00006:517,
        C1901A00006:518,
        C1901A00006:519 ;
    skos:definition "Subdivision DGeneral"@en-AU ;
    skos:narrower C1901A00006:319 ;
    skos:prefLabel "Subdivision S327"@en-AU ;
    dcat:accessURL "https://www.legislation.gov.au/C1901A00006/2024-07-01/2024-07-01/text/original/epub/OEBPS/document_1/document_1.html#_Toc172623301"^^xsd:anyURI .

