@prefix C2004A04997: <http://example.org/au/leg/dataset/C2004A04997/> .
@prefix dcat: <http://www.w3.org/ns/dcat#> .
@prefix dt: <http://purl.org/dc/terms/> .
@prefix legcons: <http://example.org/au/leg/concepts/> .
@prefix owl: <http://www.w3.org/2002/07/owl#> .
@prefix rdfs: <http://www.w3.org/2000/01/rdf-schema#> .
@prefix schema: <https://schema.org/> .
@prefix skos: <http://www.w3.org/2004/02/skos/core#> .
@prefix xsd: <http://www.w3.org/2001/XMLSchema#> .

C2004A04997: a owl:Ontology,
        dcat:Dataset ;
    dt:Agent "Home Affairs"@en-AU ;
    dt:created "2024-08-15T09:25:23.005184"^^xsd:dateTime ;
    dt:creator "https://orcid.org/0009-0007-8434-7325"^^xsd:anyURI ;
    dt:date "2024-07-01T00:00:00+10:00"^^xsd:dateTime ;
    dt:description "Customs Tariff Act 1995"@en-AU ;
    dt:identifier "https://www.legislation.gov.au/C2004A04997/latest"^^xsd:anyURI ;
    dt:publisher "Department of Home Affairs" ;
    dt:source "scheme=AGLSTERMS.AglsAgent; corporateName=Office Parliamentary Counsel; address=Locked Bag 30 Kingston ACT 2604; contact=+61 2 6120 1400"@en-AU ;
    dt:subject "Customs Tariff Act 1995"@en-AU ;
    dt:title "Customs Tariff Act 1995"@en-AU ;
    owl:imports legcons: ;
    dcat:theme legcons:ToC ;
    schema:identifier "C2004A04997" ;
    schema:status "In force" ;
    schema:version "C2024C00273 (C92)" .

C2004A04997:Endnotes a legcons:Endnotes,
        owl:Class,
        skos:Concept,
        dcat:Resource ;
    rdfs:label "Endnotes" ;
    skos:prefLabel "Endnotes" .

C2004A04997:10 a C2004A04997:Item ;
    rdfs:label "Item - I10 7  Rules for classifying goods in Schedule 3"@en-AU ;
    dt:isPartOf C2004A04997:2 ;
    rdfs:comment "7  Rules for classifying goods in Schedule 3 - Abrievated Graph Key: I10"@en-AU ;
    skos:definition "7  Rules for classifying goods in Schedule 3"@en-AU ;
    skos:narrower C2004A04997:2 ;
    skos:prefLabel "Item I10"@en-AU ;
    dcat:accessURL "https://www.legislation.gov.au/C2004A04997/2024-07-01/2024-07-01/text/1/epub/OEBPS/document_1/document_1.html#_Toc172806510"^^xsd:anyURI .

C2004A04997:100 a C2004A04997:Item ;
    rdfs:label "Item - I100 Subheading Notes"@en-AU ;
    dt:isPartOf C2004A04997:61 ;
    rdfs:comment "Subheading Notes - Abrievated Graph Key: I100"@en-AU ;
    skos:definition "Subheading Notes"@en-AU ;
    skos:narrower C2004A04997:61 ;
    skos:prefLabel "Item I100"@en-AU ;
    dcat:accessURL "https://www.legislation.gov.au/C2004A04997/2024-07-01/2024-07-01/text/1/epub/OEBPS/document_1/document_1.html#_Toc172806600"^^xsd:anyURI .

C2004A04997:101 a C2004A04997:Item ;
    rdfs:label "Item - I101 Additional Note"@en-AU ;
    dt:isPartOf C2004A04997:61 ;
    rdfs:comment "Additional Note - Abrievated Graph Key: I101"@en-AU ;
    skos:definition "Additional Note"@en-AU ;
    skos:narrower C2004A04997:61 ;
    skos:prefLabel "Item I101"@en-AU ;
    dcat:accessURL "https://www.legislation.gov.au/C2004A04997/2024-07-01/2024-07-01/text/1/epub/OEBPS/document_1/document_1.html#_Toc172806601"^^xsd:anyURI .

C2004A04997:102 a C2004A04997:Volume ;
    rdfs:label "Volume - V102 Volume 2"@en-AU ;
    dt:hasPart C2004A04997:103 ;
    rdfs:comment "Volume 2 - Abrievated Graph Key: V102"@en-AU ;
    skos:broader C2004A04997:103 ;
    skos:definition "Volume 2"@en-AU ;
    skos:prefLabel "Volume V102"@en-AU ;
    dcat:accessURL "https://www.legislation.gov.au/C2004A04997/2024-07-01/2024-07-01/text/1/epub/OEBPS/document_2/document_2.html"^^xsd:anyURI .

C2004A04997:104 a C2004A04997:Section ;
    rdfs:label "Section - S104 Section IVPrepared foodstuffs beverages spirits and vinegar tobacco and manufactured tobacco substitutes products whether or not containing nicotine intended for inhalation without combustion other nicotine containing products intended for the intake of nicotine into the human body"@en-AU ;
    dt:isPartOf C2004A04997:103 ;
    rdfs:comment "Section IVPrepared foodstuffs beverages spirits and vinegar tobacco and manufactured tobacco substitutes products whether or not containing nicotine intended for inhalation without combustion other nicotine containing products intended for the intake of nicotine into the human body - Abrievated Graph Key: S104"@en-AU ;
    skos:definition "Section IVPrepared foodstuffs beverages spirits and vinegar tobacco and manufactured tobacco substitutes products whether or not containing nicotine intended for inhalation without combustion other nicotine containing products intended for the intake of nicotine into the human body"@en-AU ;
    skos:narrower C2004A04997:103 ;
    skos:prefLabel "Section S104"@en-AU ;
    dcat:accessURL "https://www.legislation.gov.au/C2004A04997/2024-07-01/2024-07-01/text/1/epub/OEBPS/document_2/document_2.html#_Toc171750930"^^xsd:anyURI .

C2004A04997:105 a C2004A04997:Item ;
    rdfs:label "Item - I105 Note"@en-AU ;
    dt:isPartOf C2004A04997:103 ;
    rdfs:comment "Note - Abrievated Graph Key: I105"@en-AU ;
    skos:definition "Note"@en-AU ;
    skos:narrower C2004A04997:103 ;
    skos:prefLabel "Item I105"@en-AU ;
    dcat:accessURL "https://www.legislation.gov.au/C2004A04997/2024-07-01/2024-07-01/text/1/epub/OEBPS/document_2/document_2.html#_Toc171750931"^^xsd:anyURI .

C2004A04997:106 a C2004A04997:Item ;
    rdfs:label "Item - I106 Additional Note"@en-AU ;
    dt:isPartOf C2004A04997:103 ;
    rdfs:comment "Additional Note - Abrievated Graph Key: I106"@en-AU ;
    skos:definition "Additional Note"@en-AU ;
    skos:narrower C2004A04997:103 ;
    skos:prefLabel "Item I106"@en-AU ;
    dcat:accessURL "https://www.legislation.gov.au/C2004A04997/2024-07-01/2024-07-01/text/1/epub/OEBPS/document_2/document_2.html#_Toc171750932"^^xsd:anyURI .

C2004A04997:107 a C2004A04997:Chapter ;
    rdfs:label "Chapter - C107 Chapter 16 Preparations of meat of fish of crustaceans molluscs or other aquatic invertebrates or of insects"@en-AU ;
    dt:isPartOf C2004A04997:103 ;
    rdfs:comment "Chapter 16 Preparations of meat of fish of crustaceans molluscs or other aquatic invertebrates or of insects - Abrievated Graph Key: C107"@en-AU ;
    skos:definition "Chapter 16 Preparations of meat of fish of crustaceans molluscs or other aquatic invertebrates or of insects"@en-AU ;
    skos:narrower C2004A04997:103 ;
    skos:prefLabel "Chapter C107"@en-AU ;
    dcat:accessURL "https://www.legislation.gov.au/C2004A04997/2024-07-01/2024-07-01/text/1/epub/OEBPS/document_2/document_2.html#_Toc171750933"^^xsd:anyURI .

C2004A04997:108 a C2004A04997:Item ;
    rdfs:label "Item - I108 Notes"@en-AU ;
    dt:isPartOf C2004A04997:103 ;
    rdfs:comment "Notes - Abrievated Graph Key: I108"@en-AU ;
    skos:definition "Notes"@en-AU ;
    skos:narrower C2004A04997:103 ;
    skos:prefLabel "Item I108"@en-AU ;
    dcat:accessURL "https://www.legislation.gov.au/C2004A04997/2024-07-01/2024-07-01/text/1/epub/OEBPS/document_2/document_2.html#_Toc171750934"^^xsd:anyURI .

C2004A04997:109 a C2004A04997:Item ;
    rdfs:label "Item - I109 Subheading Notes"@en-AU ;
    dt:isPartOf C2004A04997:103 ;
    rdfs:comment "Subheading Notes - Abrievated Graph Key: I109"@en-AU ;
    skos:definition "Subheading Notes"@en-AU ;
    skos:narrower C2004A04997:103 ;
    skos:prefLabel "Item I109"@en-AU ;
    dcat:accessURL "https://www.legislation.gov.au/C2004A04997/2024-07-01/2024-07-01/text/1/epub/OEBPS/document_2/document_2.html#_Toc171750935"^^xsd:anyURI .

C2004A04997:11 a C2004A04997:Item ;
    rdfs:label "Item - I11 8  Application of Schedule 4"@en-AU ;
    dt:isPartOf C2004A04997:2 ;
    rdfs:comment "8  Application of Schedule 4 - Abrievated Graph Key: I11"@en-AU ;
    skos:definition "8  Application of Schedule 4"@en-AU ;
    skos:narrower C2004A04997:2 ;
    skos:prefLabel "Item I11"@en-AU ;
    dcat:accessURL "https://www.legislation.gov.au/C2004A04997/2024-07-01/2024-07-01/text/1/epub/OEBPS/document_1/document_1.html#_Toc172806511"^^xsd:anyURI .

C2004A04997:110 a C2004A04997:Chapter ;
    rdfs:label "Chapter - C110 Chapter 17 Sugars and sugar confectionery"@en-AU ;
    dt:isPartOf C2004A04997:103 ;
    rdfs:comment "Chapter 17 Sugars and sugar confectionery - Abrievated Graph Key: C110"@en-AU ;
    skos:definition "Chapter 17 Sugars and sugar confectionery"@en-AU ;
    skos:narrower C2004A04997:103 ;
    skos:prefLabel "Chapter C110"@en-AU ;
    dcat:accessURL "https://www.legislation.gov.au/C2004A04997/2024-07-01/2024-07-01/text/1/epub/OEBPS/document_2/document_2.html#_Toc171750936"^^xsd:anyURI .

C2004A04997:111 a C2004A04997:Item ;
    rdfs:label "Item - I111 Note"@en-AU ;
    dt:isPartOf C2004A04997:103 ;
    rdfs:comment "Note - Abrievated Graph Key: I111"@en-AU ;
    skos:definition "Note"@en-AU ;
    skos:narrower C2004A04997:103 ;
    skos:prefLabel "Item I111"@en-AU ;
    dcat:accessURL "https://www.legislation.gov.au/C2004A04997/2024-07-01/2024-07-01/text/1/epub/OEBPS/document_2/document_2.html#_Toc171750937"^^xsd:anyURI .

C2004A04997:112 a C2004A04997:Item ;
    rdfs:label "Item - I112 Subheading Notes"@en-AU ;
    dt:isPartOf C2004A04997:103 ;
    rdfs:comment "Subheading Notes - Abrievated Graph Key: I112"@en-AU ;
    skos:definition "Subheading Notes"@en-AU ;
    skos:narrower C2004A04997:103 ;
    skos:prefLabel "Item I112"@en-AU ;
    dcat:accessURL "https://www.legislation.gov.au/C2004A04997/2024-07-01/2024-07-01/text/1/epub/OEBPS/document_2/document_2.html#_Toc171750938"^^xsd:anyURI .

C2004A04997:113 a C2004A04997:Chapter ;
    rdfs:label "Chapter - C113 Chapter 18 Cocoa and cocoa preparations"@en-AU ;
    dt:isPartOf C2004A04997:103 ;
    rdfs:comment "Chapter 18 Cocoa and cocoa preparations - Abrievated Graph Key: C113"@en-AU ;
    skos:definition "Chapter 18 Cocoa and cocoa preparations"@en-AU ;
    skos:narrower C2004A04997:103 ;
    skos:prefLabel "Chapter C113"@en-AU ;
    dcat:accessURL "https://www.legislation.gov.au/C2004A04997/2024-07-01/2024-07-01/text/1/epub/OEBPS/document_2/document_2.html#_Toc171750939"^^xsd:anyURI .

C2004A04997:114 a C2004A04997:Item ;
    rdfs:label "Item - I114 Notes"@en-AU ;
    dt:isPartOf C2004A04997:103 ;
    rdfs:comment "Notes - Abrievated Graph Key: I114"@en-AU ;
    skos:definition "Notes"@en-AU ;
    skos:narrower C2004A04997:103 ;
    skos:prefLabel "Item I114"@en-AU ;
    dcat:accessURL "https://www.legislation.gov.au/C2004A04997/2024-07-01/2024-07-01/text/1/epub/OEBPS/document_2/document_2.html#_Toc171750940"^^xsd:anyURI .

C2004A04997:115 a C2004A04997:Chapter ;
    rdfs:label "Chapter - C115 Chapter 19 Preparations of cereals flour starch or milk pastrycooks products"@en-AU ;
    dt:isPartOf C2004A04997:103 ;
    rdfs:comment "Chapter 19 Preparations of cereals flour starch or milk pastrycooks products - Abrievated Graph Key: C115"@en-AU ;
    skos:definition "Chapter 19 Preparations of cereals flour starch or milk pastrycooks products"@en-AU ;
    skos:narrower C2004A04997:103 ;
    skos:prefLabel "Chapter C115"@en-AU ;
    dcat:accessURL "https://www.legislation.gov.au/C2004A04997/2024-07-01/2024-07-01/text/1/epub/OEBPS/document_2/document_2.html#_Toc171750941"^^xsd:anyURI .

C2004A04997:116 a C2004A04997:Item ;
    rdfs:label "Item - I116 Notes"@en-AU ;
    dt:isPartOf C2004A04997:103 ;
    rdfs:comment "Notes - Abrievated Graph Key: I116"@en-AU ;
    skos:definition "Notes"@en-AU ;
    skos:narrower C2004A04997:103 ;
    skos:prefLabel "Item I116"@en-AU ;
    dcat:accessURL "https://www.legislation.gov.au/C2004A04997/2024-07-01/2024-07-01/text/1/epub/OEBPS/document_2/document_2.html#_Toc171750942"^^xsd:anyURI .

C2004A04997:117 a C2004A04997:Item ;
    rdfs:label "Item - I117 Additional Note"@en-AU ;
    dt:isPartOf C2004A04997:103 ;
    rdfs:comment "Additional Note - Abrievated Graph Key: I117"@en-AU ;
    skos:definition "Additional Note"@en-AU ;
    skos:narrower C2004A04997:103 ;
    skos:prefLabel "Item I117"@en-AU ;
    dcat:accessURL "https://www.legislation.gov.au/C2004A04997/2024-07-01/2024-07-01/text/1/epub/OEBPS/document_2/document_2.html#_Toc171750943"^^xsd:anyURI .

C2004A04997:118 a C2004A04997:Chapter ;
    rdfs:label "Chapter - C118 Chapter 20 Preparations of vegetables fruit nuts or other parts of plants"@en-AU ;
    dt:isPartOf C2004A04997:103 ;
    rdfs:comment "Chapter 20 Preparations of vegetables fruit nuts or other parts of plants - Abrievated Graph Key: C118"@en-AU ;
    skos:definition "Chapter 20 Preparations of vegetables fruit nuts or other parts of plants"@en-AU ;
    skos:narrower C2004A04997:103 ;
    skos:prefLabel "Chapter C118"@en-AU ;
    dcat:accessURL "https://www.legislation.gov.au/C2004A04997/2024-07-01/2024-07-01/text/1/epub/OEBPS/document_2/document_2.html#_Toc171750944"^^xsd:anyURI .

C2004A04997:119 a C2004A04997:Item ;
    rdfs:label "Item - I119 Notes"@en-AU ;
    dt:isPartOf C2004A04997:103 ;
    rdfs:comment "Notes - Abrievated Graph Key: I119"@en-AU ;
    skos:definition "Notes"@en-AU ;
    skos:narrower C2004A04997:103 ;
    skos:prefLabel "Item I119"@en-AU ;
    dcat:accessURL "https://www.legislation.gov.au/C2004A04997/2024-07-01/2024-07-01/text/1/epub/OEBPS/document_2/document_2.html#_Toc171750945"^^xsd:anyURI .

C2004A04997:12 a C2004A04997:Item ;
    rdfs:label "Item - I12 9  Rates of dutyad valorem duties"@en-AU ;
    dt:isPartOf C2004A04997:2 ;
    rdfs:comment "9  Rates of dutyad valorem duties - Abrievated Graph Key: I12"@en-AU ;
    skos:definition "9  Rates of dutyad valorem duties"@en-AU ;
    skos:narrower C2004A04997:2 ;
    skos:prefLabel "Item I12"@en-AU ;
    dcat:accessURL "https://www.legislation.gov.au/C2004A04997/2024-07-01/2024-07-01/text/1/epub/OEBPS/document_1/document_1.html#_Toc172806512"^^xsd:anyURI .

C2004A04997:120 a C2004A04997:Item ;
    rdfs:label "Item - I120 Subheading Notes"@en-AU ;
    dt:isPartOf C2004A04997:103 ;
    rdfs:comment "Subheading Notes - Abrievated Graph Key: I120"@en-AU ;
    skos:definition "Subheading Notes"@en-AU ;
    skos:narrower C2004A04997:103 ;
    skos:prefLabel "Item I120"@en-AU ;
    dcat:accessURL "https://www.legislation.gov.au/C2004A04997/2024-07-01/2024-07-01/text/1/epub/OEBPS/document_2/document_2.html#_Toc171750946"^^xsd:anyURI .

C2004A04997:121 a C2004A04997:Item ;
    rdfs:label "Item - I121 Additional Notes"@en-AU ;
    dt:isPartOf C2004A04997:103 ;
    rdfs:comment "Additional Notes - Abrievated Graph Key: I121"@en-AU ;
    skos:definition "Additional Notes"@en-AU ;
    skos:narrower C2004A04997:103 ;
    skos:prefLabel "Item I121"@en-AU ;
    dcat:accessURL "https://www.legislation.gov.au/C2004A04997/2024-07-01/2024-07-01/text/1/epub/OEBPS/document_2/document_2.html#_Toc171750947"^^xsd:anyURI .

C2004A04997:122 a C2004A04997:Chapter ;
    rdfs:label "Chapter - C122 Chapter 21 Miscellaneous edible preparations"@en-AU ;
    dt:isPartOf C2004A04997:103 ;
    rdfs:comment "Chapter 21 Miscellaneous edible preparations - Abrievated Graph Key: C122"@en-AU ;
    skos:definition "Chapter 21 Miscellaneous edible preparations"@en-AU ;
    skos:narrower C2004A04997:103 ;
    skos:prefLabel "Chapter C122"@en-AU ;
    dcat:accessURL "https://www.legislation.gov.au/C2004A04997/2024-07-01/2024-07-01/text/1/epub/OEBPS/document_2/document_2.html#_Toc171750948"^^xsd:anyURI .

C2004A04997:123 a C2004A04997:Item ;
    rdfs:label "Item - I123 Notes"@en-AU ;
    dt:isPartOf C2004A04997:103 ;
    rdfs:comment "Notes - Abrievated Graph Key: I123"@en-AU ;
    skos:definition "Notes"@en-AU ;
    skos:narrower C2004A04997:103 ;
    skos:prefLabel "Item I123"@en-AU ;
    dcat:accessURL "https://www.legislation.gov.au/C2004A04997/2024-07-01/2024-07-01/text/1/epub/OEBPS/document_2/document_2.html#_Toc171750949"^^xsd:anyURI .

C2004A04997:124 a C2004A04997:Item ;
    rdfs:label "Item - I124 Additional Notes"@en-AU ;
    dt:isPartOf C2004A04997:103 ;
    rdfs:comment "Additional Notes - Abrievated Graph Key: I124"@en-AU ;
    skos:definition "Additional Notes"@en-AU ;
    skos:narrower C2004A04997:103 ;
    skos:prefLabel "Item I124"@en-AU ;
    dcat:accessURL "https://www.legislation.gov.au/C2004A04997/2024-07-01/2024-07-01/text/1/epub/OEBPS/document_2/document_2.html#_Toc171750950"^^xsd:anyURI .

C2004A04997:125 a C2004A04997:Chapter ;
    rdfs:label "Chapter - C125 Chapter 22 Beverages spirits and vinegar"@en-AU ;
    dt:isPartOf C2004A04997:103 ;
    rdfs:comment "Chapter 22 Beverages spirits and vinegar - Abrievated Graph Key: C125"@en-AU ;
    skos:definition "Chapter 22 Beverages spirits and vinegar"@en-AU ;
    skos:narrower C2004A04997:103 ;
    skos:prefLabel "Chapter C125"@en-AU ;
    dcat:accessURL "https://www.legislation.gov.au/C2004A04997/2024-07-01/2024-07-01/text/1/epub/OEBPS/document_2/document_2.html#_Toc171750951"^^xsd:anyURI .

C2004A04997:126 a C2004A04997:Item ;
    rdfs:label "Item - I126 Notes"@en-AU ;
    dt:isPartOf C2004A04997:103 ;
    rdfs:comment "Notes - Abrievated Graph Key: I126"@en-AU ;
    skos:definition "Notes"@en-AU ;
    skos:narrower C2004A04997:103 ;
    skos:prefLabel "Item I126"@en-AU ;
    dcat:accessURL "https://www.legislation.gov.au/C2004A04997/2024-07-01/2024-07-01/text/1/epub/OEBPS/document_2/document_2.html#_Toc171750952"^^xsd:anyURI .

C2004A04997:127 a C2004A04997:Item ;
    rdfs:label "Item - I127 Subheading Note"@en-AU ;
    dt:isPartOf C2004A04997:103 ;
    rdfs:comment "Subheading Note - Abrievated Graph Key: I127"@en-AU ;
    skos:definition "Subheading Note"@en-AU ;
    skos:narrower C2004A04997:103 ;
    skos:prefLabel "Item I127"@en-AU ;
    dcat:accessURL "https://www.legislation.gov.au/C2004A04997/2024-07-01/2024-07-01/text/1/epub/OEBPS/document_2/document_2.html#_Toc171750953"^^xsd:anyURI .

C2004A04997:128 a C2004A04997:Item ;
    rdfs:label "Item - I128 Additional Notes"@en-AU ;
    dt:isPartOf C2004A04997:103 ;
    rdfs:comment "Additional Notes - Abrievated Graph Key: I128"@en-AU ;
    skos:definition "Additional Notes"@en-AU ;
    skos:narrower C2004A04997:103 ;
    skos:prefLabel "Item I128"@en-AU ;
    dcat:accessURL "https://www.legislation.gov.au/C2004A04997/2024-07-01/2024-07-01/text/1/epub/OEBPS/document_2/document_2.html#_Toc171750954"^^xsd:anyURI .

C2004A04997:129 a C2004A04997:Chapter ;
    rdfs:label "Chapter - C129 Chapter 23 Residues and waste from the food industries prepared animal fodder"@en-AU ;
    dt:isPartOf C2004A04997:103 ;
    rdfs:comment "Chapter 23 Residues and waste from the food industries prepared animal fodder - Abrievated Graph Key: C129"@en-AU ;
    skos:definition "Chapter 23 Residues and waste from the food industries prepared animal fodder"@en-AU ;
    skos:narrower C2004A04997:103 ;
    skos:prefLabel "Chapter C129"@en-AU ;
    dcat:accessURL "https://www.legislation.gov.au/C2004A04997/2024-07-01/2024-07-01/text/1/epub/OEBPS/document_2/document_2.html#_Toc171750955"^^xsd:anyURI .

C2004A04997:13 a C2004A04997:Item ;
    rdfs:label "Item - I13 10  Certain words etc are rates of duty"@en-AU ;
    dt:isPartOf C2004A04997:2 ;
    rdfs:comment "10  Certain words etc are rates of duty - Abrievated Graph Key: I13"@en-AU ;
    skos:definition "10  Certain words etc are rates of duty"@en-AU ;
    skos:narrower C2004A04997:2 ;
    skos:prefLabel "Item I13"@en-AU ;
    dcat:accessURL "https://www.legislation.gov.au/C2004A04997/2024-07-01/2024-07-01/text/1/epub/OEBPS/document_1/document_1.html#_Toc172806513"^^xsd:anyURI .

C2004A04997:130 a C2004A04997:Item ;
    rdfs:label "Item - I130 Note"@en-AU ;
    dt:isPartOf C2004A04997:103 ;
    rdfs:comment "Note - Abrievated Graph Key: I130"@en-AU ;
    skos:definition "Note"@en-AU ;
    skos:narrower C2004A04997:103 ;
    skos:prefLabel "Item I130"@en-AU ;
    dcat:accessURL "https://www.legislation.gov.au/C2004A04997/2024-07-01/2024-07-01/text/1/epub/OEBPS/document_2/document_2.html#_Toc171750956"^^xsd:anyURI .

C2004A04997:131 a C2004A04997:Item ;
    rdfs:label "Item - I131 Subheading Note"@en-AU ;
    dt:isPartOf C2004A04997:103 ;
    rdfs:comment "Subheading Note - Abrievated Graph Key: I131"@en-AU ;
    skos:definition "Subheading Note"@en-AU ;
    skos:narrower C2004A04997:103 ;
    skos:prefLabel "Item I131"@en-AU ;
    dcat:accessURL "https://www.legislation.gov.au/C2004A04997/2024-07-01/2024-07-01/text/1/epub/OEBPS/document_2/document_2.html#_Toc171750957"^^xsd:anyURI .

C2004A04997:132 a C2004A04997:Chapter ;
    rdfs:label "Chapter - C132 Chapter 24 Tobacco and manufactured tobacco substitutes products whether or not containing nicotine intended for inhalation without combustion other nicotine containing products intended for the intake of nicotine into the human body"@en-AU ;
    dt:isPartOf C2004A04997:103 ;
    rdfs:comment "Chapter 24 Tobacco and manufactured tobacco substitutes products whether or not containing nicotine intended for inhalation without combustion other nicotine containing products intended for the intake of nicotine into the human body - Abrievated Graph Key: C132"@en-AU ;
    skos:definition "Chapter 24 Tobacco and manufactured tobacco substitutes products whether or not containing nicotine intended for inhalation without combustion other nicotine containing products intended for the intake of nicotine into the human body"@en-AU ;
    skos:narrower C2004A04997:103 ;
    skos:prefLabel "Chapter C132"@en-AU ;
    dcat:accessURL "https://www.legislation.gov.au/C2004A04997/2024-07-01/2024-07-01/text/1/epub/OEBPS/document_2/document_2.html#_Toc171750958"^^xsd:anyURI .

C2004A04997:133 a C2004A04997:Item ;
    rdfs:label "Item - I133 Notes"@en-AU ;
    dt:isPartOf C2004A04997:103 ;
    rdfs:comment "Notes - Abrievated Graph Key: I133"@en-AU ;
    skos:definition "Notes"@en-AU ;
    skos:narrower C2004A04997:103 ;
    skos:prefLabel "Item I133"@en-AU ;
    dcat:accessURL "https://www.legislation.gov.au/C2004A04997/2024-07-01/2024-07-01/text/1/epub/OEBPS/document_2/document_2.html#_Toc171750959"^^xsd:anyURI .

C2004A04997:134 a C2004A04997:Item ;
    rdfs:label "Item - I134 Subheading Note"@en-AU ;
    dt:isPartOf C2004A04997:103 ;
    rdfs:comment "Subheading Note - Abrievated Graph Key: I134"@en-AU ;
    skos:definition "Subheading Note"@en-AU ;
    skos:narrower C2004A04997:103 ;
    skos:prefLabel "Item I134"@en-AU ;
    dcat:accessURL "https://www.legislation.gov.au/C2004A04997/2024-07-01/2024-07-01/text/1/epub/OEBPS/document_2/document_2.html#_Toc171750960"^^xsd:anyURI .

C2004A04997:135 a C2004A04997:Item ;
    rdfs:label "Item - I135 Additional Notes"@en-AU ;
    dt:isPartOf C2004A04997:103 ;
    rdfs:comment "Additional Notes - Abrievated Graph Key: I135"@en-AU ;
    skos:definition "Additional Notes"@en-AU ;
    skos:narrower C2004A04997:103 ;
    skos:prefLabel "Item I135"@en-AU ;
    dcat:accessURL "https://www.legislation.gov.au/C2004A04997/2024-07-01/2024-07-01/text/1/epub/OEBPS/document_2/document_2.html#_Toc171750961"^^xsd:anyURI .

C2004A04997:136 a C2004A04997:Section ;
    rdfs:label "Section - S136 Section VMineral products"@en-AU ;
    dt:isPartOf C2004A04997:103 ;
    rdfs:comment "Section VMineral products - Abrievated Graph Key: S136"@en-AU ;
    skos:definition "Section VMineral products"@en-AU ;
    skos:narrower C2004A04997:103 ;
    skos:prefLabel "Section S136"@en-AU ;
    dcat:accessURL "https://www.legislation.gov.au/C2004A04997/2024-07-01/2024-07-01/text/1/epub/OEBPS/document_2/document_2.html#_Toc171750962"^^xsd:anyURI .

C2004A04997:137 a C2004A04997:Chapter ;
    rdfs:label "Chapter - C137 Chapter 25 Salt sulphur earths and stone plastering materials lime and cement"@en-AU ;
    dt:isPartOf C2004A04997:103 ;
    rdfs:comment "Chapter 25 Salt sulphur earths and stone plastering materials lime and cement - Abrievated Graph Key: C137"@en-AU ;
    skos:definition "Chapter 25 Salt sulphur earths and stone plastering materials lime and cement"@en-AU ;
    skos:narrower C2004A04997:103 ;
    skos:prefLabel "Chapter C137"@en-AU ;
    dcat:accessURL "https://www.legislation.gov.au/C2004A04997/2024-07-01/2024-07-01/text/1/epub/OEBPS/document_2/document_2.html#_Toc171750963"^^xsd:anyURI .

C2004A04997:138 a C2004A04997:Item ;
    rdfs:label "Item - I138 Notes"@en-AU ;
    dt:isPartOf C2004A04997:103 ;
    rdfs:comment "Notes - Abrievated Graph Key: I138"@en-AU ;
    skos:definition "Notes"@en-AU ;
    skos:narrower C2004A04997:103 ;
    skos:prefLabel "Item I138"@en-AU ;
    dcat:accessURL "https://www.legislation.gov.au/C2004A04997/2024-07-01/2024-07-01/text/1/epub/OEBPS/document_2/document_2.html#_Toc171750964"^^xsd:anyURI .

C2004A04997:139 a C2004A04997:Chapter ;
    rdfs:label "Chapter - C139 Chapter 26 Ores slag and ash"@en-AU ;
    dt:isPartOf C2004A04997:103 ;
    rdfs:comment "Chapter 26 Ores slag and ash - Abrievated Graph Key: C139"@en-AU ;
    skos:definition "Chapter 26 Ores slag and ash"@en-AU ;
    skos:narrower C2004A04997:103 ;
    skos:prefLabel "Chapter C139"@en-AU ;
    dcat:accessURL "https://www.legislation.gov.au/C2004A04997/2024-07-01/2024-07-01/text/1/epub/OEBPS/document_2/document_2.html#_Toc171750965"^^xsd:anyURI .

C2004A04997:14 a C2004A04997:Item ;
    rdfs:label "Item - I14 11  Rates of dutyphasing rates"@en-AU ;
    dt:isPartOf C2004A04997:2 ;
    rdfs:comment "11  Rates of dutyphasing rates - Abrievated Graph Key: I14"@en-AU ;
    skos:definition "11  Rates of dutyphasing rates"@en-AU ;
    skos:narrower C2004A04997:2 ;
    skos:prefLabel "Item I14"@en-AU ;
    dcat:accessURL "https://www.legislation.gov.au/C2004A04997/2024-07-01/2024-07-01/text/1/epub/OEBPS/document_1/document_1.html#_Toc172806514"^^xsd:anyURI .

C2004A04997:140 a C2004A04997:Item ;
    rdfs:label "Item - I140 Notes"@en-AU ;
    dt:isPartOf C2004A04997:103 ;
    rdfs:comment "Notes - Abrievated Graph Key: I140"@en-AU ;
    skos:definition "Notes"@en-AU ;
    skos:narrower C2004A04997:103 ;
    skos:prefLabel "Item I140"@en-AU ;
    dcat:accessURL "https://www.legislation.gov.au/C2004A04997/2024-07-01/2024-07-01/text/1/epub/OEBPS/document_2/document_2.html#_Toc171750966"^^xsd:anyURI .

C2004A04997:141 a C2004A04997:Item ;
    rdfs:label "Item - I141 Subheading Notes"@en-AU ;
    dt:isPartOf C2004A04997:103 ;
    rdfs:comment "Subheading Notes - Abrievated Graph Key: I141"@en-AU ;
    skos:definition "Subheading Notes"@en-AU ;
    skos:narrower C2004A04997:103 ;
    skos:prefLabel "Item I141"@en-AU ;
    dcat:accessURL "https://www.legislation.gov.au/C2004A04997/2024-07-01/2024-07-01/text/1/epub/OEBPS/document_2/document_2.html#_Toc171750967"^^xsd:anyURI .

C2004A04997:142 a C2004A04997:Chapter ;
    rdfs:label "Chapter - C142 Chapter 27 Mineral fuels mineral oils and products of their distillation bituminous substances mineral waxes"@en-AU ;
    dt:isPartOf C2004A04997:103 ;
    rdfs:comment "Chapter 27 Mineral fuels mineral oils and products of their distillation bituminous substances mineral waxes - Abrievated Graph Key: C142"@en-AU ;
    skos:definition "Chapter 27 Mineral fuels mineral oils and products of their distillation bituminous substances mineral waxes"@en-AU ;
    skos:narrower C2004A04997:103 ;
    skos:prefLabel "Chapter C142"@en-AU ;
    dcat:accessURL "https://www.legislation.gov.au/C2004A04997/2024-07-01/2024-07-01/text/1/epub/OEBPS/document_2/document_2.html#_Toc171750968"^^xsd:anyURI .

C2004A04997:143 a C2004A04997:Item ;
    rdfs:label "Item - I143 Notes"@en-AU ;
    dt:isPartOf C2004A04997:103 ;
    rdfs:comment "Notes - Abrievated Graph Key: I143"@en-AU ;
    skos:definition "Notes"@en-AU ;
    skos:narrower C2004A04997:103 ;
    skos:prefLabel "Item I143"@en-AU ;
    dcat:accessURL "https://www.legislation.gov.au/C2004A04997/2024-07-01/2024-07-01/text/1/epub/OEBPS/document_2/document_2.html#_Toc171750969"^^xsd:anyURI .

C2004A04997:144 a C2004A04997:Item ;
    rdfs:label "Item - I144 Subheading Notes"@en-AU ;
    dt:isPartOf C2004A04997:103 ;
    rdfs:comment "Subheading Notes - Abrievated Graph Key: I144"@en-AU ;
    skos:definition "Subheading Notes"@en-AU ;
    skos:narrower C2004A04997:103 ;
    skos:prefLabel "Item I144"@en-AU ;
    dcat:accessURL "https://www.legislation.gov.au/C2004A04997/2024-07-01/2024-07-01/text/1/epub/OEBPS/document_2/document_2.html#_Toc171750970"^^xsd:anyURI .

C2004A04997:145 a C2004A04997:Item ;
    rdfs:label "Item - I145 Additional Notes"@en-AU ;
    dt:isPartOf C2004A04997:103 ;
    rdfs:comment "Additional Notes - Abrievated Graph Key: I145"@en-AU ;
    skos:definition "Additional Notes"@en-AU ;
    skos:narrower C2004A04997:103 ;
    skos:prefLabel "Item I145"@en-AU ;
    dcat:accessURL "https://www.legislation.gov.au/C2004A04997/2024-07-01/2024-07-01/text/1/epub/OEBPS/document_2/document_2.html#_Toc171750971"^^xsd:anyURI .

C2004A04997:146 a C2004A04997:Section ;
    rdfs:label "Section - S146 Section VIProducts of the chemical or allied industries"@en-AU ;
    dt:isPartOf C2004A04997:103 ;
    rdfs:comment "Section VIProducts of the chemical or allied industries - Abrievated Graph Key: S146"@en-AU ;
    skos:definition "Section VIProducts of the chemical or allied industries"@en-AU ;
    skos:narrower C2004A04997:103 ;
    skos:prefLabel "Section S146"@en-AU ;
    dcat:accessURL "https://www.legislation.gov.au/C2004A04997/2024-07-01/2024-07-01/text/1/epub/OEBPS/document_2/document_2.html#_Toc171750972"^^xsd:anyURI .

C2004A04997:147 a C2004A04997:Item ;
    rdfs:label "Item - I147 Notes"@en-AU ;
    dt:isPartOf C2004A04997:103 ;
    rdfs:comment "Notes - Abrievated Graph Key: I147"@en-AU ;
    skos:definition "Notes"@en-AU ;
    skos:narrower C2004A04997:103 ;
    skos:prefLabel "Item I147"@en-AU ;
    dcat:accessURL "https://www.legislation.gov.au/C2004A04997/2024-07-01/2024-07-01/text/1/epub/OEBPS/document_2/document_2.html#_Toc171750973"^^xsd:anyURI .

C2004A04997:148 a C2004A04997:Chapter ;
    rdfs:label "Chapter - C148 Chapter 28 Inorganic chemicals organic or inorganic compounds of precious metals of rare earth metals of radioactive elements or of isotopes"@en-AU ;
    dt:isPartOf C2004A04997:103 ;
    rdfs:comment "Chapter 28 Inorganic chemicals organic or inorganic compounds of precious metals of rare earth metals of radioactive elements or of isotopes - Abrievated Graph Key: C148"@en-AU ;
    skos:definition "Chapter 28 Inorganic chemicals organic or inorganic compounds of precious metals of rare earth metals of radioactive elements or of isotopes"@en-AU ;
    skos:narrower C2004A04997:103 ;
    skos:prefLabel "Chapter C148"@en-AU ;
    dcat:accessURL "https://www.legislation.gov.au/C2004A04997/2024-07-01/2024-07-01/text/1/epub/OEBPS/document_2/document_2.html#_Toc171750974"^^xsd:anyURI .

C2004A04997:149 a C2004A04997:Item ;
    rdfs:label "Item - I149 Notes"@en-AU ;
    dt:isPartOf C2004A04997:103 ;
    rdfs:comment "Notes - Abrievated Graph Key: I149"@en-AU ;
    skos:definition "Notes"@en-AU ;
    skos:narrower C2004A04997:103 ;
    skos:prefLabel "Item I149"@en-AU ;
    dcat:accessURL "https://www.legislation.gov.au/C2004A04997/2024-07-01/2024-07-01/text/1/epub/OEBPS/document_2/document_2.html#_Toc171750975"^^xsd:anyURI .

C2004A04997:15 a C2004A04997:Item ;
    rdfs:label "Item - I15 12  Classes of countries and places in relation to which special rates apply"@en-AU ;
    dt:isPartOf C2004A04997:2 ;
    rdfs:comment "12  Classes of countries and places in relation to which special rates apply - Abrievated Graph Key: I15"@en-AU ;
    skos:definition "12  Classes of countries and places in relation to which special rates apply"@en-AU ;
    skos:narrower C2004A04997:2 ;
    skos:prefLabel "Item I15"@en-AU ;
    dcat:accessURL "https://www.legislation.gov.au/C2004A04997/2024-07-01/2024-07-01/text/1/epub/OEBPS/document_1/document_1.html#_Toc172806515"^^xsd:anyURI .

C2004A04997:150 a C2004A04997:Item ;
    rdfs:label "Item - I150 Subheading Note"@en-AU ;
    dt:isPartOf C2004A04997:103 ;
    rdfs:comment "Subheading Note - Abrievated Graph Key: I150"@en-AU ;
    skos:definition "Subheading Note"@en-AU ;
    skos:narrower C2004A04997:103 ;
    skos:prefLabel "Item I150"@en-AU ;
    dcat:accessURL "https://www.legislation.gov.au/C2004A04997/2024-07-01/2024-07-01/text/1/epub/OEBPS/document_2/document_2.html#_Toc171750976"^^xsd:anyURI .

C2004A04997:151 a C2004A04997:Item ;
    rdfs:label "Item - I151 Additional Note"@en-AU ;
    dt:isPartOf C2004A04997:103 ;
    rdfs:comment "Additional Note - Abrievated Graph Key: I151"@en-AU ;
    skos:definition "Additional Note"@en-AU ;
    skos:narrower C2004A04997:103 ;
    skos:prefLabel "Item I151"@en-AU ;
    dcat:accessURL "https://www.legislation.gov.au/C2004A04997/2024-07-01/2024-07-01/text/1/epub/OEBPS/document_2/document_2.html#_Toc171750977"^^xsd:anyURI .

C2004A04997:152 a C2004A04997:Item ;
    rdfs:label "Item - I152 Sub Chapter IChemical elements"@en-AU ;
    dt:isPartOf C2004A04997:103 ;
    rdfs:comment "Sub Chapter IChemical elements - Abrievated Graph Key: I152"@en-AU ;
    skos:definition "Sub Chapter IChemical elements"@en-AU ;
    skos:narrower C2004A04997:103 ;
    skos:prefLabel "Item I152"@en-AU ;
    dcat:accessURL "https://www.legislation.gov.au/C2004A04997/2024-07-01/2024-07-01/text/1/epub/OEBPS/document_2/document_2.html#_Toc171750978"^^xsd:anyURI .

C2004A04997:153 a C2004A04997:Item ;
    rdfs:label "Item - I153 Sub Chapter IIInorganic acids and inorganic oxygen compounds of non metals"@en-AU ;
    dt:isPartOf C2004A04997:103 ;
    rdfs:comment "Sub Chapter IIInorganic acids and inorganic oxygen compounds of non metals - Abrievated Graph Key: I153"@en-AU ;
    skos:definition "Sub Chapter IIInorganic acids and inorganic oxygen compounds of non metals"@en-AU ;
    skos:narrower C2004A04997:103 ;
    skos:prefLabel "Item I153"@en-AU ;
    dcat:accessURL "https://www.legislation.gov.au/C2004A04997/2024-07-01/2024-07-01/text/1/epub/OEBPS/document_2/document_2.html#_Toc171750979"^^xsd:anyURI .

C2004A04997:154 a C2004A04997:Item ;
    rdfs:label "Item - I154 Sub Chapter IIIHalogen or sulphur compounds of non metals"@en-AU ;
    dt:isPartOf C2004A04997:103 ;
    rdfs:comment "Sub Chapter IIIHalogen or sulphur compounds of non metals - Abrievated Graph Key: I154"@en-AU ;
    skos:definition "Sub Chapter IIIHalogen or sulphur compounds of non metals"@en-AU ;
    skos:narrower C2004A04997:103 ;
    skos:prefLabel "Item I154"@en-AU ;
    dcat:accessURL "https://www.legislation.gov.au/C2004A04997/2024-07-01/2024-07-01/text/1/epub/OEBPS/document_2/document_2.html#_Toc171750980"^^xsd:anyURI .

C2004A04997:155 a C2004A04997:Item ;
    rdfs:label "Item - I155 Sub Chapter IVInorganic bases and oxides hydroxides and peroxides of metal"@en-AU ;
    dt:isPartOf C2004A04997:103 ;
    rdfs:comment "Sub Chapter IVInorganic bases and oxides hydroxides and peroxides of metal - Abrievated Graph Key: I155"@en-AU ;
    skos:definition "Sub Chapter IVInorganic bases and oxides hydroxides and peroxides of metal"@en-AU ;
    skos:narrower C2004A04997:103 ;
    skos:prefLabel "Item I155"@en-AU ;
    dcat:accessURL "https://www.legislation.gov.au/C2004A04997/2024-07-01/2024-07-01/text/1/epub/OEBPS/document_2/document_2.html#_Toc171750981"^^xsd:anyURI .

C2004A04997:156 a C2004A04997:Item ;
    rdfs:label "Item - I156 Sub Chapter VSalts and peroxysalts of inorganic acids and metals"@en-AU ;
    dt:isPartOf C2004A04997:103 ;
    rdfs:comment "Sub Chapter VSalts and peroxysalts of inorganic acids and metals - Abrievated Graph Key: I156"@en-AU ;
    skos:definition "Sub Chapter VSalts and peroxysalts of inorganic acids and metals"@en-AU ;
    skos:narrower C2004A04997:103 ;
    skos:prefLabel "Item I156"@en-AU ;
    dcat:accessURL "https://www.legislation.gov.au/C2004A04997/2024-07-01/2024-07-01/text/1/epub/OEBPS/document_2/document_2.html#_Toc171750982"^^xsd:anyURI .

C2004A04997:157 a C2004A04997:Item ;
    rdfs:label "Item - I157 Sub Chapter VIMiscellaneous"@en-AU ;
    dt:isPartOf C2004A04997:103 ;
    rdfs:comment "Sub Chapter VIMiscellaneous - Abrievated Graph Key: I157"@en-AU ;
    skos:definition "Sub Chapter VIMiscellaneous"@en-AU ;
    skos:narrower C2004A04997:103 ;
    skos:prefLabel "Item I157"@en-AU ;
    dcat:accessURL "https://www.legislation.gov.au/C2004A04997/2024-07-01/2024-07-01/text/1/epub/OEBPS/document_2/document_2.html#_Toc171750983"^^xsd:anyURI .

C2004A04997:158 a C2004A04997:Chapter ;
    rdfs:label "Chapter - C158 Chapter 29 Organic chemicals"@en-AU ;
    dt:isPartOf C2004A04997:103 ;
    rdfs:comment "Chapter 29 Organic chemicals - Abrievated Graph Key: C158"@en-AU ;
    skos:definition "Chapter 29 Organic chemicals"@en-AU ;
    skos:narrower C2004A04997:103 ;
    skos:prefLabel "Chapter C158"@en-AU ;
    dcat:accessURL "https://www.legislation.gov.au/C2004A04997/2024-07-01/2024-07-01/text/1/epub/OEBPS/document_2/document_2.html#_Toc171750984"^^xsd:anyURI .

C2004A04997:159 a C2004A04997:Item ;
    rdfs:label "Item - I159 Notes"@en-AU ;
    dt:isPartOf C2004A04997:103 ;
    rdfs:comment "Notes - Abrievated Graph Key: I159"@en-AU ;
    skos:definition "Notes"@en-AU ;
    skos:narrower C2004A04997:103 ;
    skos:prefLabel "Item I159"@en-AU ;
    dcat:accessURL "https://www.legislation.gov.au/C2004A04997/2024-07-01/2024-07-01/text/1/epub/OEBPS/document_2/document_2.html#_Toc171750985"^^xsd:anyURI .

C2004A04997:16 a C2004A04997:Item ;
    rdfs:label "Item - I16 13  When goods are the produce or manufacture of a particular country or place"@en-AU ;
    dt:isPartOf C2004A04997:2 ;
    rdfs:comment "13  When goods are the produce or manufacture of a particular country or place - Abrievated Graph Key: I16"@en-AU ;
    skos:definition "13  When goods are the produce or manufacture of a particular country or place"@en-AU ;
    skos:narrower C2004A04997:2 ;
    skos:prefLabel "Item I16"@en-AU ;
    dcat:accessURL "https://www.legislation.gov.au/C2004A04997/2024-07-01/2024-07-01/text/1/epub/OEBPS/document_1/document_1.html#_Toc172806516"^^xsd:anyURI .

C2004A04997:160 a C2004A04997:Item ;
    rdfs:label "Item - I160 Subheading Notes"@en-AU ;
    dt:isPartOf C2004A04997:103 ;
    rdfs:comment "Subheading Notes - Abrievated Graph Key: I160"@en-AU ;
    skos:definition "Subheading Notes"@en-AU ;
    skos:narrower C2004A04997:103 ;
    skos:prefLabel "Item I160"@en-AU ;
    dcat:accessURL "https://www.legislation.gov.au/C2004A04997/2024-07-01/2024-07-01/text/1/epub/OEBPS/document_2/document_2.html#_Toc171750986"^^xsd:anyURI .

C2004A04997:161 a C2004A04997:Item ;
    rdfs:label "Item - I161 Additional Note"@en-AU ;
    dt:isPartOf C2004A04997:103 ;
    rdfs:comment "Additional Note - Abrievated Graph Key: I161"@en-AU ;
    skos:definition "Additional Note"@en-AU ;
    skos:narrower C2004A04997:103 ;
    skos:prefLabel "Item I161"@en-AU ;
    dcat:accessURL "https://www.legislation.gov.au/C2004A04997/2024-07-01/2024-07-01/text/1/epub/OEBPS/document_2/document_2.html#_Toc171750987"^^xsd:anyURI .

C2004A04997:162 a C2004A04997:Item ;
    rdfs:label "Item - I162 Sub Chapter IHydrocarbons and their halogenated sulphonated nitrated or nitrosated derivatives"@en-AU ;
    dt:isPartOf C2004A04997:103 ;
    rdfs:comment "Sub Chapter IHydrocarbons and their halogenated sulphonated nitrated or nitrosated derivatives - Abrievated Graph Key: I162"@en-AU ;
    skos:definition "Sub Chapter IHydrocarbons and their halogenated sulphonated nitrated or nitrosated derivatives"@en-AU ;
    skos:narrower C2004A04997:103 ;
    skos:prefLabel "Item I162"@en-AU ;
    dcat:accessURL "https://www.legislation.gov.au/C2004A04997/2024-07-01/2024-07-01/text/1/epub/OEBPS/document_2/document_2.html#_Toc171750988"^^xsd:anyURI .

C2004A04997:163 a C2004A04997:Item ;
    rdfs:label "Item - I163 Sub Chapter IIAlcohols and their halogenated sulphonated nitrated or nitrosated derivatives"@en-AU ;
    dt:isPartOf C2004A04997:103 ;
    rdfs:comment "Sub Chapter IIAlcohols and their halogenated sulphonated nitrated or nitrosated derivatives - Abrievated Graph Key: I163"@en-AU ;
    skos:definition "Sub Chapter IIAlcohols and their halogenated sulphonated nitrated or nitrosated derivatives"@en-AU ;
    skos:narrower C2004A04997:103 ;
    skos:prefLabel "Item I163"@en-AU ;
    dcat:accessURL "https://www.legislation.gov.au/C2004A04997/2024-07-01/2024-07-01/text/1/epub/OEBPS/document_2/document_2.html#_Toc171750989"^^xsd:anyURI .

C2004A04997:164 a C2004A04997:Item ;
    rdfs:label "Item - I164 Sub Chapter IIIPhenols phenol alcohols and their halogenated sulphonated nitrated or nitrosated derivatives"@en-AU ;
    dt:isPartOf C2004A04997:103 ;
    rdfs:comment "Sub Chapter IIIPhenols phenol alcohols and their halogenated sulphonated nitrated or nitrosated derivatives - Abrievated Graph Key: I164"@en-AU ;
    skos:definition "Sub Chapter IIIPhenols phenol alcohols and their halogenated sulphonated nitrated or nitrosated derivatives"@en-AU ;
    skos:narrower C2004A04997:103 ;
    skos:prefLabel "Item I164"@en-AU ;
    dcat:accessURL "https://www.legislation.gov.au/C2004A04997/2024-07-01/2024-07-01/text/1/epub/OEBPS/document_2/document_2.html#_Toc171750990"^^xsd:anyURI .

C2004A04997:165 a C2004A04997:Item ;
    rdfs:label "Item - I165 Sub Chapter IVEthers alcohol peroxides ether peroxides acetal and hemiacetal peroxides ketone peroxides epoxides with a three membered ring acetals and hemiacetals and their halogenated sulphonated nitrated or nitrosated derivatives"@en-AU ;
    dt:isPartOf C2004A04997:103 ;
    rdfs:comment "Sub Chapter IVEthers alcohol peroxides ether peroxides acetal and hemiacetal peroxides ketone peroxides epoxides with a three membered ring acetals and hemiacetals and their halogenated sulphonated nitrated or nitrosated derivatives - Abrievated Graph Key: I165"@en-AU ;
    skos:definition "Sub Chapter IVEthers alcohol peroxides ether peroxides acetal and hemiacetal peroxides ketone peroxides epoxides with a three membered ring acetals and hemiacetals and their halogenated sulphonated nitrated or nitrosated derivatives"@en-AU ;
    skos:narrower C2004A04997:103 ;
    skos:prefLabel "Item I165"@en-AU ;
    dcat:accessURL "https://www.legislation.gov.au/C2004A04997/2024-07-01/2024-07-01/text/1/epub/OEBPS/document_2/document_2.html#_Toc171750991"^^xsd:anyURI .

C2004A04997:166 a C2004A04997:Item ;
    rdfs:label "Item - I166 Sub Chapter VAldehyde function compounds"@en-AU ;
    dt:isPartOf C2004A04997:103 ;
    rdfs:comment "Sub Chapter VAldehyde function compounds - Abrievated Graph Key: I166"@en-AU ;
    skos:definition "Sub Chapter VAldehyde function compounds"@en-AU ;
    skos:narrower C2004A04997:103 ;
    skos:prefLabel "Item I166"@en-AU ;
    dcat:accessURL "https://www.legislation.gov.au/C2004A04997/2024-07-01/2024-07-01/text/1/epub/OEBPS/document_2/document_2.html#_Toc171750992"^^xsd:anyURI .

C2004A04997:167 a C2004A04997:Item ;
    rdfs:label "Item - I167 Sub Chapter VIKetone function compounds and quinone function compounds"@en-AU ;
    dt:isPartOf C2004A04997:103 ;
    rdfs:comment "Sub Chapter VIKetone function compounds and quinone function compounds - Abrievated Graph Key: I167"@en-AU ;
    skos:definition "Sub Chapter VIKetone function compounds and quinone function compounds"@en-AU ;
    skos:narrower C2004A04997:103 ;
    skos:prefLabel "Item I167"@en-AU ;
    dcat:accessURL "https://www.legislation.gov.au/C2004A04997/2024-07-01/2024-07-01/text/1/epub/OEBPS/document_2/document_2.html#_Toc171750993"^^xsd:anyURI .

C2004A04997:168 a C2004A04997:Item ;
    rdfs:label "Item - I168 Sub Chapter VIICarboxylic acids and their anhydrides halides peroxides and peroxyacids and their halogenated sulphonated nitrated or nitrosated derivatives"@en-AU ;
    dt:isPartOf C2004A04997:103 ;
    rdfs:comment "Sub Chapter VIICarboxylic acids and their anhydrides halides peroxides and peroxyacids and their halogenated sulphonated nitrated or nitrosated derivatives - Abrievated Graph Key: I168"@en-AU ;
    skos:definition "Sub Chapter VIICarboxylic acids and their anhydrides halides peroxides and peroxyacids and their halogenated sulphonated nitrated or nitrosated derivatives"@en-AU ;
    skos:narrower C2004A04997:103 ;
    skos:prefLabel "Item I168"@en-AU ;
    dcat:accessURL "https://www.legislation.gov.au/C2004A04997/2024-07-01/2024-07-01/text/1/epub/OEBPS/document_2/document_2.html#_Toc171750994"^^xsd:anyURI .

C2004A04997:169 a C2004A04997:Item ;
    rdfs:label "Item - I169 Sub Chapter VIIIEsters of inorganic acids of non metals and their salts and their halogenated sulphonated nitrated or nitrosated derivatives"@en-AU ;
    dt:isPartOf C2004A04997:103 ;
    rdfs:comment "Sub Chapter VIIIEsters of inorganic acids of non metals and their salts and their halogenated sulphonated nitrated or nitrosated derivatives - Abrievated Graph Key: I169"@en-AU ;
    skos:definition "Sub Chapter VIIIEsters of inorganic acids of non metals and their salts and their halogenated sulphonated nitrated or nitrosated derivatives"@en-AU ;
    skos:narrower C2004A04997:103 ;
    skos:prefLabel "Item I169"@en-AU ;
    dcat:accessURL "https://www.legislation.gov.au/C2004A04997/2024-07-01/2024-07-01/text/1/epub/OEBPS/document_2/document_2.html#_Toc171750995"^^xsd:anyURI .

C2004A04997:17 a C2004A04997:Item ;
    rdfs:label "Item - I17 13 AA  When goods are Singaporean originating goods"@en-AU ;
    dt:isPartOf C2004A04997:2 ;
    rdfs:comment "13 AA  When goods are Singaporean originating goods - Abrievated Graph Key: I17"@en-AU ;
    skos:definition "13 AA  When goods are Singaporean originating goods"@en-AU ;
    skos:narrower C2004A04997:2 ;
    skos:prefLabel "Item I17"@en-AU ;
    dcat:accessURL "https://www.legislation.gov.au/C2004A04997/2024-07-01/2024-07-01/text/1/epub/OEBPS/document_1/document_1.html#_Toc172806517"^^xsd:anyURI .

C2004A04997:170 a C2004A04997:Item ;
    rdfs:label "Item - I170 Sub Chapter IXNitrogen function compounds"@en-AU ;
    dt:isPartOf C2004A04997:103 ;
    rdfs:comment "Sub Chapter IXNitrogen function compounds - Abrievated Graph Key: I170"@en-AU ;
    skos:definition "Sub Chapter IXNitrogen function compounds"@en-AU ;
    skos:narrower C2004A04997:103 ;
    skos:prefLabel "Item I170"@en-AU ;
    dcat:accessURL "https://www.legislation.gov.au/C2004A04997/2024-07-01/2024-07-01/text/1/epub/OEBPS/document_2/document_2.html#_Toc171750996"^^xsd:anyURI .

C2004A04997:171 a C2004A04997:Item ;
    rdfs:label "Item - I171 Sub Chapter XOrgano inorganic compounds heterocyclic compounds nucleic acids and their salts and sulphonamides"@en-AU ;
    dt:isPartOf C2004A04997:103 ;
    rdfs:comment "Sub Chapter XOrgano inorganic compounds heterocyclic compounds nucleic acids and their salts and sulphonamides - Abrievated Graph Key: I171"@en-AU ;
    skos:definition "Sub Chapter XOrgano inorganic compounds heterocyclic compounds nucleic acids and their salts and sulphonamides"@en-AU ;
    skos:narrower C2004A04997:103 ;
    skos:prefLabel "Item I171"@en-AU ;
    dcat:accessURL "https://www.legislation.gov.au/C2004A04997/2024-07-01/2024-07-01/text/1/epub/OEBPS/document_2/document_2.html#_Toc171750997"^^xsd:anyURI .

C2004A04997:172 a C2004A04997:Item ;
    rdfs:label "Item - I172 Sub Chapter XIProvitamins vitamins and hormones"@en-AU ;
    dt:isPartOf C2004A04997:103 ;
    rdfs:comment "Sub Chapter XIProvitamins vitamins and hormones - Abrievated Graph Key: I172"@en-AU ;
    skos:definition "Sub Chapter XIProvitamins vitamins and hormones"@en-AU ;
    skos:narrower C2004A04997:103 ;
    skos:prefLabel "Item I172"@en-AU ;
    dcat:accessURL "https://www.legislation.gov.au/C2004A04997/2024-07-01/2024-07-01/text/1/epub/OEBPS/document_2/document_2.html#_Toc171750998"^^xsd:anyURI .

C2004A04997:173 a C2004A04997:Item ;
    rdfs:label "Item - I173 Sub Chapter XIIGlycosides and alkaloids natural or reproduced by synthesis and their salts ethers esters and other derivatives"@en-AU ;
    dt:isPartOf C2004A04997:103 ;
    rdfs:comment "Sub Chapter XIIGlycosides and alkaloids natural or reproduced by synthesis and their salts ethers esters and other derivatives - Abrievated Graph Key: I173"@en-AU ;
    skos:definition "Sub Chapter XIIGlycosides and alkaloids natural or reproduced by synthesis and their salts ethers esters and other derivatives"@en-AU ;
    skos:narrower C2004A04997:103 ;
    skos:prefLabel "Item I173"@en-AU ;
    dcat:accessURL "https://www.legislation.gov.au/C2004A04997/2024-07-01/2024-07-01/text/1/epub/OEBPS/document_2/document_2.html#_Toc171750999"^^xsd:anyURI .

C2004A04997:174 a C2004A04997:Item ;
    rdfs:label "Item - I174 Sub Chapter XIIIOther organic compounds"@en-AU ;
    dt:isPartOf C2004A04997:103 ;
    rdfs:comment "Sub Chapter XIIIOther organic compounds - Abrievated Graph Key: I174"@en-AU ;
    skos:definition "Sub Chapter XIIIOther organic compounds"@en-AU ;
    skos:narrower C2004A04997:103 ;
    skos:prefLabel "Item I174"@en-AU ;
    dcat:accessURL "https://www.legislation.gov.au/C2004A04997/2024-07-01/2024-07-01/text/1/epub/OEBPS/document_2/document_2.html#_Toc171751000"^^xsd:anyURI .

C2004A04997:175 a C2004A04997:Chapter ;
    rdfs:label "Chapter - C175 Chapter 30 Pharmaceutical products"@en-AU ;
    dt:isPartOf C2004A04997:103 ;
    rdfs:comment "Chapter 30 Pharmaceutical products - Abrievated Graph Key: C175"@en-AU ;
    skos:definition "Chapter 30 Pharmaceutical products"@en-AU ;
    skos:narrower C2004A04997:103 ;
    skos:prefLabel "Chapter C175"@en-AU ;
    dcat:accessURL "https://www.legislation.gov.au/C2004A04997/2024-07-01/2024-07-01/text/1/epub/OEBPS/document_2/document_2.html#_Toc171751001"^^xsd:anyURI .

C2004A04997:176 a C2004A04997:Item ;
    rdfs:label "Item - I176 Notes"@en-AU ;
    dt:isPartOf C2004A04997:103 ;
    rdfs:comment "Notes - Abrievated Graph Key: I176"@en-AU ;
    skos:definition "Notes"@en-AU ;
    skos:narrower C2004A04997:103 ;
    skos:prefLabel "Item I176"@en-AU ;
    dcat:accessURL "https://www.legislation.gov.au/C2004A04997/2024-07-01/2024-07-01/text/1/epub/OEBPS/document_2/document_2.html#_Toc171751002"^^xsd:anyURI .

C2004A04997:177 a C2004A04997:Item ;
    rdfs:label "Item - I177 Subheading Notes"@en-AU ;
    dt:isPartOf C2004A04997:103 ;
    rdfs:comment "Subheading Notes - Abrievated Graph Key: I177"@en-AU ;
    skos:definition "Subheading Notes"@en-AU ;
    skos:narrower C2004A04997:103 ;
    skos:prefLabel "Item I177"@en-AU ;
    dcat:accessURL "https://www.legislation.gov.au/C2004A04997/2024-07-01/2024-07-01/text/1/epub/OEBPS/document_2/document_2.html#_Toc171751003"^^xsd:anyURI .

C2004A04997:178 a C2004A04997:Item ;
    rdfs:label "Item - I178 Additional Notes"@en-AU ;
    dt:isPartOf C2004A04997:103 ;
    rdfs:comment "Additional Notes - Abrievated Graph Key: I178"@en-AU ;
    skos:definition "Additional Notes"@en-AU ;
    skos:narrower C2004A04997:103 ;
    skos:prefLabel "Item I178"@en-AU ;
    dcat:accessURL "https://www.legislation.gov.au/C2004A04997/2024-07-01/2024-07-01/text/1/epub/OEBPS/document_2/document_2.html#_Toc171751004"^^xsd:anyURI .

C2004A04997:179 a C2004A04997:Chapter ;
    rdfs:label "Chapter - C179 Chapter 31 Fertilisers"@en-AU ;
    dt:isPartOf C2004A04997:103 ;
    rdfs:comment "Chapter 31 Fertilisers - Abrievated Graph Key: C179"@en-AU ;
    skos:definition "Chapter 31 Fertilisers"@en-AU ;
    skos:narrower C2004A04997:103 ;
    skos:prefLabel "Chapter C179"@en-AU ;
    dcat:accessURL "https://www.legislation.gov.au/C2004A04997/2024-07-01/2024-07-01/text/1/epub/OEBPS/document_2/document_2.html#_Toc171751005"^^xsd:anyURI .

C2004A04997:18 a C2004A04997:Item ;
    rdfs:label "Item - I18 13 A  When goods are US originating goods"@en-AU ;
    dt:isPartOf C2004A04997:2 ;
    rdfs:comment "13 A  When goods are US originating goods - Abrievated Graph Key: I18"@en-AU ;
    skos:definition "13 A  When goods are US originating goods"@en-AU ;
    skos:narrower C2004A04997:2 ;
    skos:prefLabel "Item I18"@en-AU ;
    dcat:accessURL "https://www.legislation.gov.au/C2004A04997/2024-07-01/2024-07-01/text/1/epub/OEBPS/document_1/document_1.html#_Toc172806518"^^xsd:anyURI .

C2004A04997:180 a C2004A04997:Item ;
    rdfs:label "Item - I180 Notes"@en-AU ;
    dt:isPartOf C2004A04997:103 ;
    rdfs:comment "Notes - Abrievated Graph Key: I180"@en-AU ;
    skos:definition "Notes"@en-AU ;
    skos:narrower C2004A04997:103 ;
    skos:prefLabel "Item I180"@en-AU ;
    dcat:accessURL "https://www.legislation.gov.au/C2004A04997/2024-07-01/2024-07-01/text/1/epub/OEBPS/document_2/document_2.html#_Toc171751006"^^xsd:anyURI .

C2004A04997:181 a C2004A04997:Chapter ;
    rdfs:label "Chapter - C181 Chapter 32 Tanning or dyeing extracts tannins and their derivatives dyes pigments and other colouring matter paints and varnishes putty and other mastics inks"@en-AU ;
    dt:isPartOf C2004A04997:103 ;
    rdfs:comment "Chapter 32 Tanning or dyeing extracts tannins and their derivatives dyes pigments and other colouring matter paints and varnishes putty and other mastics inks - Abrievated Graph Key: C181"@en-AU ;
    skos:definition "Chapter 32 Tanning or dyeing extracts tannins and their derivatives dyes pigments and other colouring matter paints and varnishes putty and other mastics inks"@en-AU ;
    skos:narrower C2004A04997:103 ;
    skos:prefLabel "Chapter C181"@en-AU ;
    dcat:accessURL "https://www.legislation.gov.au/C2004A04997/2024-07-01/2024-07-01/text/1/epub/OEBPS/document_2/document_2.html#_Toc171751007"^^xsd:anyURI .

C2004A04997:182 a C2004A04997:Item ;
    rdfs:label "Item - I182 Notes"@en-AU ;
    dt:isPartOf C2004A04997:103 ;
    rdfs:comment "Notes - Abrievated Graph Key: I182"@en-AU ;
    skos:definition "Notes"@en-AU ;
    skos:narrower C2004A04997:103 ;
    skos:prefLabel "Item I182"@en-AU ;
    dcat:accessURL "https://www.legislation.gov.au/C2004A04997/2024-07-01/2024-07-01/text/1/epub/OEBPS/document_2/document_2.html#_Toc171751008"^^xsd:anyURI .

C2004A04997:183 a C2004A04997:Chapter ;
    rdfs:label "Chapter - C183 Chapter 33 Essential oils and resinoids perfumery cosmetic or toilet preparations"@en-AU ;
    dt:isPartOf C2004A04997:103 ;
    rdfs:comment "Chapter 33 Essential oils and resinoids perfumery cosmetic or toilet preparations - Abrievated Graph Key: C183"@en-AU ;
    skos:definition "Chapter 33 Essential oils and resinoids perfumery cosmetic or toilet preparations"@en-AU ;
    skos:narrower C2004A04997:103 ;
    skos:prefLabel "Chapter C183"@en-AU ;
    dcat:accessURL "https://www.legislation.gov.au/C2004A04997/2024-07-01/2024-07-01/text/1/epub/OEBPS/document_2/document_2.html#_Toc171751009"^^xsd:anyURI .

C2004A04997:184 a C2004A04997:Item ;
    rdfs:label "Item - I184 Notes"@en-AU ;
    dt:isPartOf C2004A04997:103 ;
    rdfs:comment "Notes - Abrievated Graph Key: I184"@en-AU ;
    skos:definition "Notes"@en-AU ;
    skos:narrower C2004A04997:103 ;
    skos:prefLabel "Item I184"@en-AU ;
    dcat:accessURL "https://www.legislation.gov.au/C2004A04997/2024-07-01/2024-07-01/text/1/epub/OEBPS/document_2/document_2.html#_Toc171751010"^^xsd:anyURI .

C2004A04997:185 a C2004A04997:Chapter ;
    rdfs:label "Chapter - C185 Chapter 34 Soap organic surface active agents washing preparations lubricating preparations artificial waxes prepared waxes polishing or scouring preparations candles and similar articles modelling pastes dental waxes and dental preparations with a basis of plaster"@en-AU ;
    dt:isPartOf C2004A04997:103 ;
    rdfs:comment "Chapter 34 Soap organic surface active agents washing preparations lubricating preparations artificial waxes prepared waxes polishing or scouring preparations candles and similar articles modelling pastes dental waxes and dental preparations with a basis of plaster - Abrievated Graph Key: C185"@en-AU ;
    skos:definition "Chapter 34 Soap organic surface active agents washing preparations lubricating preparations artificial waxes prepared waxes polishing or scouring preparations candles and similar articles modelling pastes dental waxes and dental preparations with a basis of plaster"@en-AU ;
    skos:narrower C2004A04997:103 ;
    skos:prefLabel "Chapter C185"@en-AU ;
    dcat:accessURL "https://www.legislation.gov.au/C2004A04997/2024-07-01/2024-07-01/text/1/epub/OEBPS/document_2/document_2.html#_Toc171751011"^^xsd:anyURI .

C2004A04997:186 a C2004A04997:Item ;
    rdfs:label "Item - I186 Notes"@en-AU ;
    dt:isPartOf C2004A04997:103 ;
    rdfs:comment "Notes - Abrievated Graph Key: I186"@en-AU ;
    skos:definition "Notes"@en-AU ;
    skos:narrower C2004A04997:103 ;
    skos:prefLabel "Item I186"@en-AU ;
    dcat:accessURL "https://www.legislation.gov.au/C2004A04997/2024-07-01/2024-07-01/text/1/epub/OEBPS/document_2/document_2.html#_Toc171751012"^^xsd:anyURI .

C2004A04997:187 a C2004A04997:Chapter ;
    rdfs:label "Chapter - C187 Chapter 35 Albuminoidal substances modified starches glues enzymes"@en-AU ;
    dt:isPartOf C2004A04997:103 ;
    rdfs:comment "Chapter 35 Albuminoidal substances modified starches glues enzymes - Abrievated Graph Key: C187"@en-AU ;
    skos:definition "Chapter 35 Albuminoidal substances modified starches glues enzymes"@en-AU ;
    skos:narrower C2004A04997:103 ;
    skos:prefLabel "Chapter C187"@en-AU ;
    dcat:accessURL "https://www.legislation.gov.au/C2004A04997/2024-07-01/2024-07-01/text/1/epub/OEBPS/document_2/document_2.html#_Toc171751013"^^xsd:anyURI .

C2004A04997:188 a C2004A04997:Item ;
    rdfs:label "Item - I188 Notes"@en-AU ;
    dt:isPartOf C2004A04997:103 ;
    rdfs:comment "Notes - Abrievated Graph Key: I188"@en-AU ;
    skos:definition "Notes"@en-AU ;
    skos:narrower C2004A04997:103 ;
    skos:prefLabel "Item I188"@en-AU ;
    dcat:accessURL "https://www.legislation.gov.au/C2004A04997/2024-07-01/2024-07-01/text/1/epub/OEBPS/document_2/document_2.html#_Toc171751014"^^xsd:anyURI .

C2004A04997:189 a C2004A04997:Chapter ;
    rdfs:label "Chapter - C189 Chapter 36 Explosives pyrotechnic products matches pyrophoric alloys certain combustible preparations"@en-AU ;
    dt:isPartOf C2004A04997:103 ;
    rdfs:comment "Chapter 36 Explosives pyrotechnic products matches pyrophoric alloys certain combustible preparations - Abrievated Graph Key: C189"@en-AU ;
    skos:definition "Chapter 36 Explosives pyrotechnic products matches pyrophoric alloys certain combustible preparations"@en-AU ;
    skos:narrower C2004A04997:103 ;
    skos:prefLabel "Chapter C189"@en-AU ;
    dcat:accessURL "https://www.legislation.gov.au/C2004A04997/2024-07-01/2024-07-01/text/1/epub/OEBPS/document_2/document_2.html#_Toc171751015"^^xsd:anyURI .

C2004A04997:19 a C2004A04997:Item ;
    rdfs:label "Item - I19 13 B  When goods are Thai originating goods"@en-AU ;
    dt:isPartOf C2004A04997:2 ;
    rdfs:comment "13 B  When goods are Thai originating goods - Abrievated Graph Key: I19"@en-AU ;
    skos:definition "13 B  When goods are Thai originating goods"@en-AU ;
    skos:narrower C2004A04997:2 ;
    skos:prefLabel "Item I19"@en-AU ;
    dcat:accessURL "https://www.legislation.gov.au/C2004A04997/2024-07-01/2024-07-01/text/1/epub/OEBPS/document_1/document_1.html#_Toc172806519"^^xsd:anyURI .

C2004A04997:190 a C2004A04997:Item ;
    rdfs:label "Item - I190 Notes"@en-AU ;
    dt:isPartOf C2004A04997:103 ;
    rdfs:comment "Notes - Abrievated Graph Key: I190"@en-AU ;
    skos:definition "Notes"@en-AU ;
    skos:narrower C2004A04997:103 ;
    skos:prefLabel "Item I190"@en-AU ;
    dcat:accessURL "https://www.legislation.gov.au/C2004A04997/2024-07-01/2024-07-01/text/1/epub/OEBPS/document_2/document_2.html#_Toc171751016"^^xsd:anyURI .

C2004A04997:191 a C2004A04997:Chapter ;
    rdfs:label "Chapter - C191 Chapter 37 Photographic or cinematographic goods"@en-AU ;
    dt:isPartOf C2004A04997:103 ;
    rdfs:comment "Chapter 37 Photographic or cinematographic goods - Abrievated Graph Key: C191"@en-AU ;
    skos:definition "Chapter 37 Photographic or cinematographic goods"@en-AU ;
    skos:narrower C2004A04997:103 ;
    skos:prefLabel "Chapter C191"@en-AU ;
    dcat:accessURL "https://www.legislation.gov.au/C2004A04997/2024-07-01/2024-07-01/text/1/epub/OEBPS/document_2/document_2.html#_Toc171751017"^^xsd:anyURI .

C2004A04997:192 a C2004A04997:Item ;
    rdfs:label "Item - I192 Notes"@en-AU ;
    dt:isPartOf C2004A04997:103 ;
    rdfs:comment "Notes - Abrievated Graph Key: I192"@en-AU ;
    skos:definition "Notes"@en-AU ;
    skos:narrower C2004A04997:103 ;
    skos:prefLabel "Item I192"@en-AU ;
    dcat:accessURL "https://www.legislation.gov.au/C2004A04997/2024-07-01/2024-07-01/text/1/epub/OEBPS/document_2/document_2.html#_Toc171751018"^^xsd:anyURI .

C2004A04997:193 a C2004A04997:Chapter ;
    rdfs:label "Chapter - C193 Chapter 38 Miscellaneous chemical products"@en-AU ;
    dt:isPartOf C2004A04997:103 ;
    rdfs:comment "Chapter 38 Miscellaneous chemical products - Abrievated Graph Key: C193"@en-AU ;
    skos:definition "Chapter 38 Miscellaneous chemical products"@en-AU ;
    skos:narrower C2004A04997:103 ;
    skos:prefLabel "Chapter C193"@en-AU ;
    dcat:accessURL "https://www.legislation.gov.au/C2004A04997/2024-07-01/2024-07-01/text/1/epub/OEBPS/document_2/document_2.html#_Toc171751019"^^xsd:anyURI .

C2004A04997:194 a C2004A04997:Item ;
    rdfs:label "Item - I194 Notes"@en-AU ;
    dt:isPartOf C2004A04997:103 ;
    rdfs:comment "Notes - Abrievated Graph Key: I194"@en-AU ;
    skos:definition "Notes"@en-AU ;
    skos:narrower C2004A04997:103 ;
    skos:prefLabel "Item I194"@en-AU ;
    dcat:accessURL "https://www.legislation.gov.au/C2004A04997/2024-07-01/2024-07-01/text/1/epub/OEBPS/document_2/document_2.html#_Toc171751020"^^xsd:anyURI .

C2004A04997:195 a C2004A04997:Item ;
    rdfs:label "Item - I195 Subheading Notes"@en-AU ;
    dt:isPartOf C2004A04997:103 ;
    rdfs:comment "Subheading Notes - Abrievated Graph Key: I195"@en-AU ;
    skos:definition "Subheading Notes"@en-AU ;
    skos:narrower C2004A04997:103 ;
    skos:prefLabel "Item I195"@en-AU ;
    dcat:accessURL "https://www.legislation.gov.au/C2004A04997/2024-07-01/2024-07-01/text/1/epub/OEBPS/document_2/document_2.html#_Toc171751021"^^xsd:anyURI .

C2004A04997:196 a C2004A04997:Item ;
    rdfs:label "Item - I196 Additional Note"@en-AU ;
    dt:isPartOf C2004A04997:103 ;
    rdfs:comment "Additional Note - Abrievated Graph Key: I196"@en-AU ;
    skos:definition "Additional Note"@en-AU ;
    skos:narrower C2004A04997:103 ;
    skos:prefLabel "Item I196"@en-AU ;
    dcat:accessURL "https://www.legislation.gov.au/C2004A04997/2024-07-01/2024-07-01/text/1/epub/OEBPS/document_2/document_2.html#_Toc171751022"^^xsd:anyURI .

C2004A04997:197 a C2004A04997:Volume ;
    rdfs:label "Volume - V197 Volume 3"@en-AU ;
    dt:hasPart C2004A04997:198 ;
    rdfs:comment "Volume 3 - Abrievated Graph Key: V197"@en-AU ;
    skos:broader C2004A04997:198 ;
    skos:definition "Volume 3"@en-AU ;
    skos:prefLabel "Volume V197"@en-AU ;
    dcat:accessURL "https://www.legislation.gov.au/C2004A04997/2024-07-01/2024-07-01/text/1/epub/OEBPS/document_3/document_3.html"^^xsd:anyURI .

C2004A04997:199 a C2004A04997:Section ;
    rdfs:label "Section - S199 Section VIIPlastics and articles thereof rubber and articles thereof"@en-AU ;
    dt:isPartOf C2004A04997:198 ;
    rdfs:comment "Section VIIPlastics and articles thereof rubber and articles thereof - Abrievated Graph Key: S199"@en-AU ;
    skos:definition "Section VIIPlastics and articles thereof rubber and articles thereof"@en-AU ;
    skos:narrower C2004A04997:198 ;
    skos:prefLabel "Section S199"@en-AU ;
    dcat:accessURL "https://www.legislation.gov.au/C2004A04997/2024-07-01/2024-07-01/text/1/epub/OEBPS/document_3/document_3.html#_Toc171751529"^^xsd:anyURI .

C2004A04997:20 a C2004A04997:Item ;
    rdfs:label "Item - I20 13 C  When goods are New Zealand originating goods"@en-AU ;
    dt:isPartOf C2004A04997:2 ;
    rdfs:comment "13 C  When goods are New Zealand originating goods - Abrievated Graph Key: I20"@en-AU ;
    skos:definition "13 C  When goods are New Zealand originating goods"@en-AU ;
    skos:narrower C2004A04997:2 ;
    skos:prefLabel "Item I20"@en-AU ;
    dcat:accessURL "https://www.legislation.gov.au/C2004A04997/2024-07-01/2024-07-01/text/1/epub/OEBPS/document_1/document_1.html#_Toc172806520"^^xsd:anyURI .

C2004A04997:200 a C2004A04997:Item ;
    rdfs:label "Item - I200 Notes"@en-AU ;
    dt:isPartOf C2004A04997:198 ;
    rdfs:comment "Notes - Abrievated Graph Key: I200"@en-AU ;
    skos:definition "Notes"@en-AU ;
    skos:narrower C2004A04997:198 ;
    skos:prefLabel "Item I200"@en-AU ;
    dcat:accessURL "https://www.legislation.gov.au/C2004A04997/2024-07-01/2024-07-01/text/1/epub/OEBPS/document_3/document_3.html#_Toc171751530"^^xsd:anyURI .

C2004A04997:201 a C2004A04997:Item ;
    rdfs:label "Item - I201 Additional Note"@en-AU ;
    dt:isPartOf C2004A04997:198 ;
    rdfs:comment "Additional Note - Abrievated Graph Key: I201"@en-AU ;
    skos:definition "Additional Note"@en-AU ;
    skos:narrower C2004A04997:198 ;
    skos:prefLabel "Item I201"@en-AU ;
    dcat:accessURL "https://www.legislation.gov.au/C2004A04997/2024-07-01/2024-07-01/text/1/epub/OEBPS/document_3/document_3.html#_Toc171751531"^^xsd:anyURI .

C2004A04997:202 a C2004A04997:Chapter ;
    rdfs:label "Chapter - C202 Chapter 39 Plastics and articles thereof"@en-AU ;
    dt:isPartOf C2004A04997:198 ;
    rdfs:comment "Chapter 39 Plastics and articles thereof - Abrievated Graph Key: C202"@en-AU ;
    skos:definition "Chapter 39 Plastics and articles thereof"@en-AU ;
    skos:narrower C2004A04997:198 ;
    skos:prefLabel "Chapter C202"@en-AU ;
    dcat:accessURL "https://www.legislation.gov.au/C2004A04997/2024-07-01/2024-07-01/text/1/epub/OEBPS/document_3/document_3.html#_Toc171751532"^^xsd:anyURI .

C2004A04997:203 a C2004A04997:Item ;
    rdfs:label "Item - I203 Notes"@en-AU ;
    dt:isPartOf C2004A04997:198 ;
    rdfs:comment "Notes - Abrievated Graph Key: I203"@en-AU ;
    skos:definition "Notes"@en-AU ;
    skos:narrower C2004A04997:198 ;
    skos:prefLabel "Item I203"@en-AU ;
    dcat:accessURL "https://www.legislation.gov.au/C2004A04997/2024-07-01/2024-07-01/text/1/epub/OEBPS/document_3/document_3.html#_Toc171751533"^^xsd:anyURI .

C2004A04997:204 a C2004A04997:Item ;
    rdfs:label "Item - I204 Subheading Notes"@en-AU ;
    dt:isPartOf C2004A04997:198 ;
    rdfs:comment "Subheading Notes - Abrievated Graph Key: I204"@en-AU ;
    skos:definition "Subheading Notes"@en-AU ;
    skos:narrower C2004A04997:198 ;
    skos:prefLabel "Item I204"@en-AU ;
    dcat:accessURL "https://www.legislation.gov.au/C2004A04997/2024-07-01/2024-07-01/text/1/epub/OEBPS/document_3/document_3.html#_Toc171751534"^^xsd:anyURI .

C2004A04997:205 a C2004A04997:Item ;
    rdfs:label "Item - I205 Additional Notes"@en-AU ;
    dt:isPartOf C2004A04997:198 ;
    rdfs:comment "Additional Notes - Abrievated Graph Key: I205"@en-AU ;
    skos:definition "Additional Notes"@en-AU ;
    skos:narrower C2004A04997:198 ;
    skos:prefLabel "Item I205"@en-AU ;
    dcat:accessURL "https://www.legislation.gov.au/C2004A04997/2024-07-01/2024-07-01/text/1/epub/OEBPS/document_3/document_3.html#_Toc171751535"^^xsd:anyURI .

C2004A04997:206 a C2004A04997:Item ;
    rdfs:label "Item - I206 Sub Chapter IPrimary forms"@en-AU ;
    dt:isPartOf C2004A04997:198 ;
    rdfs:comment "Sub Chapter IPrimary forms - Abrievated Graph Key: I206"@en-AU ;
    skos:definition "Sub Chapter IPrimary forms"@en-AU ;
    skos:narrower C2004A04997:198 ;
    skos:prefLabel "Item I206"@en-AU ;
    dcat:accessURL "https://www.legislation.gov.au/C2004A04997/2024-07-01/2024-07-01/text/1/epub/OEBPS/document_3/document_3.html#_Toc171751536"^^xsd:anyURI .

C2004A04997:207 a C2004A04997:Item ;
    rdfs:label "Item - I207 Sub Chapter IIWaste parings and scrap semi manufactures articles"@en-AU ;
    dt:isPartOf C2004A04997:198 ;
    rdfs:comment "Sub Chapter IIWaste parings and scrap semi manufactures articles - Abrievated Graph Key: I207"@en-AU ;
    skos:definition "Sub Chapter IIWaste parings and scrap semi manufactures articles"@en-AU ;
    skos:narrower C2004A04997:198 ;
    skos:prefLabel "Item I207"@en-AU ;
    dcat:accessURL "https://www.legislation.gov.au/C2004A04997/2024-07-01/2024-07-01/text/1/epub/OEBPS/document_3/document_3.html#_Toc171751537"^^xsd:anyURI .

C2004A04997:208 a C2004A04997:Chapter ;
    rdfs:label "Chapter - C208 Chapter 40 Rubber and articles thereof"@en-AU ;
    dt:isPartOf C2004A04997:198 ;
    rdfs:comment "Chapter 40 Rubber and articles thereof - Abrievated Graph Key: C208"@en-AU ;
    skos:definition "Chapter 40 Rubber and articles thereof"@en-AU ;
    skos:narrower C2004A04997:198 ;
    skos:prefLabel "Chapter C208"@en-AU ;
    dcat:accessURL "https://www.legislation.gov.au/C2004A04997/2024-07-01/2024-07-01/text/1/epub/OEBPS/document_3/document_3.html#_Toc171751538"^^xsd:anyURI .

C2004A04997:209 a C2004A04997:Item ;
    rdfs:label "Item - I209 Notes"@en-AU ;
    dt:isPartOf C2004A04997:198 ;
    rdfs:comment "Notes - Abrievated Graph Key: I209"@en-AU ;
    skos:definition "Notes"@en-AU ;
    skos:narrower C2004A04997:198 ;
    skos:prefLabel "Item I209"@en-AU ;
    dcat:accessURL "https://www.legislation.gov.au/C2004A04997/2024-07-01/2024-07-01/text/1/epub/OEBPS/document_3/document_3.html#_Toc171751539"^^xsd:anyURI .

C2004A04997:21 a C2004A04997:Item ;
    rdfs:label "Item - I21 13 CA  When goods are Peruvian originating goods"@en-AU ;
    dt:isPartOf C2004A04997:2 ;
    rdfs:comment "13 CA  When goods are Peruvian originating goods - Abrievated Graph Key: I21"@en-AU ;
    skos:definition "13 CA  When goods are Peruvian originating goods"@en-AU ;
    skos:narrower C2004A04997:2 ;
    skos:prefLabel "Item I21"@en-AU ;
    dcat:accessURL "https://www.legislation.gov.au/C2004A04997/2024-07-01/2024-07-01/text/1/epub/OEBPS/document_1/document_1.html#_Toc172806521"^^xsd:anyURI .

C2004A04997:210 a C2004A04997:Section ;
    rdfs:label "Section - S210 Section VIIIRaw hides and skins leather furskins and articles thereof saddlery and harness travel goods handbags and similar containers articles of animal gut other than silk worm gut"@en-AU ;
    dt:isPartOf C2004A04997:198 ;
    rdfs:comment "Section VIIIRaw hides and skins leather furskins and articles thereof saddlery and harness travel goods handbags and similar containers articles of animal gut other than silk worm gut - Abrievated Graph Key: S210"@en-AU ;
    skos:definition "Section VIIIRaw hides and skins leather furskins and articles thereof saddlery and harness travel goods handbags and similar containers articles of animal gut other than silk worm gut"@en-AU ;
    skos:narrower C2004A04997:198 ;
    skos:prefLabel "Section S210"@en-AU ;
    dcat:accessURL "https://www.legislation.gov.au/C2004A04997/2024-07-01/2024-07-01/text/1/epub/OEBPS/document_3/document_3.html#_Toc171751540"^^xsd:anyURI .

C2004A04997:211 a C2004A04997:Chapter ;
    rdfs:label "Chapter - C211 Chapter 41 Raw hides and skins other than furskins and leather"@en-AU ;
    dt:isPartOf C2004A04997:198 ;
    rdfs:comment "Chapter 41 Raw hides and skins other than furskins and leather - Abrievated Graph Key: C211"@en-AU ;
    skos:definition "Chapter 41 Raw hides and skins other than furskins and leather"@en-AU ;
    skos:narrower C2004A04997:198 ;
    skos:prefLabel "Chapter C211"@en-AU ;
    dcat:accessURL "https://www.legislation.gov.au/C2004A04997/2024-07-01/2024-07-01/text/1/epub/OEBPS/document_3/document_3.html#_Toc171751541"^^xsd:anyURI .

C2004A04997:212 a C2004A04997:Item ;
    rdfs:label "Item - I212 Notes"@en-AU ;
    dt:isPartOf C2004A04997:198 ;
    rdfs:comment "Notes - Abrievated Graph Key: I212"@en-AU ;
    skos:definition "Notes"@en-AU ;
    skos:narrower C2004A04997:198 ;
    skos:prefLabel "Item I212"@en-AU ;
    dcat:accessURL "https://www.legislation.gov.au/C2004A04997/2024-07-01/2024-07-01/text/1/epub/OEBPS/document_3/document_3.html#_Toc171751542"^^xsd:anyURI .

C2004A04997:213 a C2004A04997:Chapter ;
    rdfs:label "Chapter - C213 Chapter 42 Articles of leather saddlery and harness travel goods handbags and similar containers articles of animal gut other than silk worm gut"@en-AU ;
    dt:isPartOf C2004A04997:198 ;
    rdfs:comment "Chapter 42 Articles of leather saddlery and harness travel goods handbags and similar containers articles of animal gut other than silk worm gut - Abrievated Graph Key: C213"@en-AU ;
    skos:definition "Chapter 42 Articles of leather saddlery and harness travel goods handbags and similar containers articles of animal gut other than silk worm gut"@en-AU ;
    skos:narrower C2004A04997:198 ;
    skos:prefLabel "Chapter C213"@en-AU ;
    dcat:accessURL "https://www.legislation.gov.au/C2004A04997/2024-07-01/2024-07-01/text/1/epub/OEBPS/document_3/document_3.html#_Toc171751543"^^xsd:anyURI .

C2004A04997:214 a C2004A04997:Item ;
    rdfs:label "Item - I214 Notes"@en-AU ;
    dt:isPartOf C2004A04997:198 ;
    rdfs:comment "Notes - Abrievated Graph Key: I214"@en-AU ;
    skos:definition "Notes"@en-AU ;
    skos:narrower C2004A04997:198 ;
    skos:prefLabel "Item I214"@en-AU ;
    dcat:accessURL "https://www.legislation.gov.au/C2004A04997/2024-07-01/2024-07-01/text/1/epub/OEBPS/document_3/document_3.html#_Toc171751544"^^xsd:anyURI .

C2004A04997:215 a C2004A04997:Chapter ;
    rdfs:label "Chapter - C215 Chapter 43 Furskins and artificial fur manufactures thereof"@en-AU ;
    dt:isPartOf C2004A04997:198 ;
    rdfs:comment "Chapter 43 Furskins and artificial fur manufactures thereof - Abrievated Graph Key: C215"@en-AU ;
    skos:definition "Chapter 43 Furskins and artificial fur manufactures thereof"@en-AU ;
    skos:narrower C2004A04997:198 ;
    skos:prefLabel "Chapter C215"@en-AU ;
    dcat:accessURL "https://www.legislation.gov.au/C2004A04997/2024-07-01/2024-07-01/text/1/epub/OEBPS/document_3/document_3.html#_Toc171751545"^^xsd:anyURI .

C2004A04997:216 a C2004A04997:Item ;
    rdfs:label "Item - I216 Notes"@en-AU ;
    dt:isPartOf C2004A04997:198 ;
    rdfs:comment "Notes - Abrievated Graph Key: I216"@en-AU ;
    skos:definition "Notes"@en-AU ;
    skos:narrower C2004A04997:198 ;
    skos:prefLabel "Item I216"@en-AU ;
    dcat:accessURL "https://www.legislation.gov.au/C2004A04997/2024-07-01/2024-07-01/text/1/epub/OEBPS/document_3/document_3.html#_Toc171751546"^^xsd:anyURI .

C2004A04997:217 a C2004A04997:Section ;
    rdfs:label "Section - S217 Section IXWood and articles of wood wood charcoal cork and articles of cork manufactures of straw of esparto or of other plaiting materials basketware and wickerwork"@en-AU ;
    dt:isPartOf C2004A04997:198 ;
    rdfs:comment "Section IXWood and articles of wood wood charcoal cork and articles of cork manufactures of straw of esparto or of other plaiting materials basketware and wickerwork - Abrievated Graph Key: S217"@en-AU ;
    skos:definition "Section IXWood and articles of wood wood charcoal cork and articles of cork manufactures of straw of esparto or of other plaiting materials basketware and wickerwork"@en-AU ;
    skos:narrower C2004A04997:198 ;
    skos:prefLabel "Section S217"@en-AU ;
    dcat:accessURL "https://www.legislation.gov.au/C2004A04997/2024-07-01/2024-07-01/text/1/epub/OEBPS/document_3/document_3.html#_Toc171751547"^^xsd:anyURI .

C2004A04997:218 a C2004A04997:Chapter ;
    rdfs:label "Chapter - C218 Chapter 44 Wood and articles of wood wood charcoal"@en-AU ;
    dt:isPartOf C2004A04997:198 ;
    rdfs:comment "Chapter 44 Wood and articles of wood wood charcoal - Abrievated Graph Key: C218"@en-AU ;
    skos:definition "Chapter 44 Wood and articles of wood wood charcoal"@en-AU ;
    skos:narrower C2004A04997:198 ;
    skos:prefLabel "Chapter C218"@en-AU ;
    dcat:accessURL "https://www.legislation.gov.au/C2004A04997/2024-07-01/2024-07-01/text/1/epub/OEBPS/document_3/document_3.html#_Toc171751548"^^xsd:anyURI .

C2004A04997:219 a C2004A04997:Item ;
    rdfs:label "Item - I219 Notes"@en-AU ;
    dt:isPartOf C2004A04997:198 ;
    rdfs:comment "Notes - Abrievated Graph Key: I219"@en-AU ;
    skos:definition "Notes"@en-AU ;
    skos:narrower C2004A04997:198 ;
    skos:prefLabel "Item I219"@en-AU ;
    dcat:accessURL "https://www.legislation.gov.au/C2004A04997/2024-07-01/2024-07-01/text/1/epub/OEBPS/document_3/document_3.html#_Toc171751549"^^xsd:anyURI .

C2004A04997:22 a C2004A04997:Item ;
    rdfs:label "Item - I22 13 D  When goods are Chilean originating goods"@en-AU ;
    dt:isPartOf C2004A04997:2 ;
    rdfs:comment "13 D  When goods are Chilean originating goods - Abrievated Graph Key: I22"@en-AU ;
    skos:definition "13 D  When goods are Chilean originating goods"@en-AU ;
    skos:narrower C2004A04997:2 ;
    skos:prefLabel "Item I22"@en-AU ;
    dcat:accessURL "https://www.legislation.gov.au/C2004A04997/2024-07-01/2024-07-01/text/1/epub/OEBPS/document_1/document_1.html#_Toc172806522"^^xsd:anyURI .

C2004A04997:220 a C2004A04997:Item ;
    rdfs:label "Item - I220 Subheading Notes"@en-AU ;
    dt:isPartOf C2004A04997:198 ;
    rdfs:comment "Subheading Notes - Abrievated Graph Key: I220"@en-AU ;
    skos:definition "Subheading Notes"@en-AU ;
    skos:narrower C2004A04997:198 ;
    skos:prefLabel "Item I220"@en-AU ;
    dcat:accessURL "https://www.legislation.gov.au/C2004A04997/2024-07-01/2024-07-01/text/1/epub/OEBPS/document_3/document_3.html#_Toc171751550"^^xsd:anyURI .

C2004A04997:221 a C2004A04997:Item ;
    rdfs:label "Item - I221 Additional Notes"@en-AU ;
    dt:isPartOf C2004A04997:198 ;
    rdfs:comment "Additional Notes - Abrievated Graph Key: I221"@en-AU ;
    skos:definition "Additional Notes"@en-AU ;
    skos:narrower C2004A04997:198 ;
    skos:prefLabel "Item I221"@en-AU ;
    dcat:accessURL "https://www.legislation.gov.au/C2004A04997/2024-07-01/2024-07-01/text/1/epub/OEBPS/document_3/document_3.html#_Toc171751551"^^xsd:anyURI .

C2004A04997:222 a C2004A04997:Chapter ;
    rdfs:label "Chapter - C222 Chapter 45 Cork and articles of cork"@en-AU ;
    dt:isPartOf C2004A04997:198 ;
    rdfs:comment "Chapter 45 Cork and articles of cork - Abrievated Graph Key: C222"@en-AU ;
    skos:definition "Chapter 45 Cork and articles of cork"@en-AU ;
    skos:narrower C2004A04997:198 ;
    skos:prefLabel "Chapter C222"@en-AU ;
    dcat:accessURL "https://www.legislation.gov.au/C2004A04997/2024-07-01/2024-07-01/text/1/epub/OEBPS/document_3/document_3.html#_Toc171751552"^^xsd:anyURI .

C2004A04997:223 a C2004A04997:Item ;
    rdfs:label "Item - I223 Note"@en-AU ;
    dt:isPartOf C2004A04997:198 ;
    rdfs:comment "Note - Abrievated Graph Key: I223"@en-AU ;
    skos:definition "Note"@en-AU ;
    skos:narrower C2004A04997:198 ;
    skos:prefLabel "Item I223"@en-AU ;
    dcat:accessURL "https://www.legislation.gov.au/C2004A04997/2024-07-01/2024-07-01/text/1/epub/OEBPS/document_3/document_3.html#_Toc171751553"^^xsd:anyURI .

C2004A04997:224 a C2004A04997:Chapter ;
    rdfs:label "Chapter - C224 Chapter 46 Manufactures of straw of esparto or of other plaiting materials basketware and wickerwork"@en-AU ;
    dt:isPartOf C2004A04997:198 ;
    rdfs:comment "Chapter 46 Manufactures of straw of esparto or of other plaiting materials basketware and wickerwork - Abrievated Graph Key: C224"@en-AU ;
    skos:definition "Chapter 46 Manufactures of straw of esparto or of other plaiting materials basketware and wickerwork"@en-AU ;
    skos:narrower C2004A04997:198 ;
    skos:prefLabel "Chapter C224"@en-AU ;
    dcat:accessURL "https://www.legislation.gov.au/C2004A04997/2024-07-01/2024-07-01/text/1/epub/OEBPS/document_3/document_3.html#_Toc171751554"^^xsd:anyURI .

C2004A04997:225 a C2004A04997:Item ;
    rdfs:label "Item - I225 Notes"@en-AU ;
    dt:isPartOf C2004A04997:198 ;
    rdfs:comment "Notes - Abrievated Graph Key: I225"@en-AU ;
    skos:definition "Notes"@en-AU ;
    skos:narrower C2004A04997:198 ;
    skos:prefLabel "Item I225"@en-AU ;
    dcat:accessURL "https://www.legislation.gov.au/C2004A04997/2024-07-01/2024-07-01/text/1/epub/OEBPS/document_3/document_3.html#_Toc171751555"^^xsd:anyURI .

C2004A04997:226 a C2004A04997:Section ;
    rdfs:label "Section - S226 Section XPulp of wood or of other fibrous cellulosic material recovered waste and scrap paper or paperboard paper and paperboard and articles thereof"@en-AU ;
    dt:isPartOf C2004A04997:198 ;
    rdfs:comment "Section XPulp of wood or of other fibrous cellulosic material recovered waste and scrap paper or paperboard paper and paperboard and articles thereof - Abrievated Graph Key: S226"@en-AU ;
    skos:definition "Section XPulp of wood or of other fibrous cellulosic material recovered waste and scrap paper or paperboard paper and paperboard and articles thereof"@en-AU ;
    skos:narrower C2004A04997:198 ;
    skos:prefLabel "Section S226"@en-AU ;
    dcat:accessURL "https://www.legislation.gov.au/C2004A04997/2024-07-01/2024-07-01/text/1/epub/OEBPS/document_3/document_3.html#_Toc171751556"^^xsd:anyURI .

C2004A04997:227 a C2004A04997:Chapter ;
    rdfs:label "Chapter - C227 Chapter 47 Pulp of wood or of other fibrous cellulosic material recovered waste and scrap paper or paperboard"@en-AU ;
    dt:isPartOf C2004A04997:198 ;
    rdfs:comment "Chapter 47 Pulp of wood or of other fibrous cellulosic material recovered waste and scrap paper or paperboard - Abrievated Graph Key: C227"@en-AU ;
    skos:definition "Chapter 47 Pulp of wood or of other fibrous cellulosic material recovered waste and scrap paper or paperboard"@en-AU ;
    skos:narrower C2004A04997:198 ;
    skos:prefLabel "Chapter C227"@en-AU ;
    dcat:accessURL "https://www.legislation.gov.au/C2004A04997/2024-07-01/2024-07-01/text/1/epub/OEBPS/document_3/document_3.html#_Toc171751557"^^xsd:anyURI .

C2004A04997:228 a C2004A04997:Item ;
    rdfs:label "Item - I228 Note"@en-AU ;
    dt:isPartOf C2004A04997:198 ;
    rdfs:comment "Note - Abrievated Graph Key: I228"@en-AU ;
    skos:definition "Note"@en-AU ;
    skos:narrower C2004A04997:198 ;
    skos:prefLabel "Item I228"@en-AU ;
    dcat:accessURL "https://www.legislation.gov.au/C2004A04997/2024-07-01/2024-07-01/text/1/epub/OEBPS/document_3/document_3.html#_Toc171751558"^^xsd:anyURI .

C2004A04997:229 a C2004A04997:Chapter ;
    rdfs:label "Chapter - C229 Chapter 48 Paper and paperboard articles of paper pulp of paper or of paperboard"@en-AU ;
    dt:isPartOf C2004A04997:198 ;
    rdfs:comment "Chapter 48 Paper and paperboard articles of paper pulp of paper or of paperboard - Abrievated Graph Key: C229"@en-AU ;
    skos:definition "Chapter 48 Paper and paperboard articles of paper pulp of paper or of paperboard"@en-AU ;
    skos:narrower C2004A04997:198 ;
    skos:prefLabel "Chapter C229"@en-AU ;
    dcat:accessURL "https://www.legislation.gov.au/C2004A04997/2024-07-01/2024-07-01/text/1/epub/OEBPS/document_3/document_3.html#_Toc171751559"^^xsd:anyURI .

C2004A04997:23 a C2004A04997:Item ;
    rdfs:label "Item - I23 13 E  When goods are ASEAN Australia New Zealand AANZ originating goods"@en-AU ;
    dt:isPartOf C2004A04997:2 ;
    rdfs:comment "13 E  When goods are ASEAN Australia New Zealand AANZ originating goods - Abrievated Graph Key: I23"@en-AU ;
    skos:definition "13 E  When goods are ASEAN Australia New Zealand AANZ originating goods"@en-AU ;
    skos:narrower C2004A04997:2 ;
    skos:prefLabel "Item I23"@en-AU ;
    dcat:accessURL "https://www.legislation.gov.au/C2004A04997/2024-07-01/2024-07-01/text/1/epub/OEBPS/document_1/document_1.html#_Toc172806523"^^xsd:anyURI .

C2004A04997:230 a C2004A04997:Item ;
    rdfs:label "Item - I230 Notes"@en-AU ;
    dt:isPartOf C2004A04997:198 ;
    rdfs:comment "Notes - Abrievated Graph Key: I230"@en-AU ;
    skos:definition "Notes"@en-AU ;
    skos:narrower C2004A04997:198 ;
    skos:prefLabel "Item I230"@en-AU ;
    dcat:accessURL "https://www.legislation.gov.au/C2004A04997/2024-07-01/2024-07-01/text/1/epub/OEBPS/document_3/document_3.html#_Toc171751560"^^xsd:anyURI .

C2004A04997:231 a C2004A04997:Item ;
    rdfs:label "Item - I231 Subheading Notes"@en-AU ;
    dt:isPartOf C2004A04997:198 ;
    rdfs:comment "Subheading Notes - Abrievated Graph Key: I231"@en-AU ;
    skos:definition "Subheading Notes"@en-AU ;
    skos:narrower C2004A04997:198 ;
    skos:prefLabel "Item I231"@en-AU ;
    dcat:accessURL "https://www.legislation.gov.au/C2004A04997/2024-07-01/2024-07-01/text/1/epub/OEBPS/document_3/document_3.html#_Toc171751561"^^xsd:anyURI .

C2004A04997:232 a C2004A04997:Item ;
    rdfs:label "Item - I232 Additional Notes"@en-AU ;
    dt:isPartOf C2004A04997:198 ;
    rdfs:comment "Additional Notes - Abrievated Graph Key: I232"@en-AU ;
    skos:definition "Additional Notes"@en-AU ;
    skos:narrower C2004A04997:198 ;
    skos:prefLabel "Item I232"@en-AU ;
    dcat:accessURL "https://www.legislation.gov.au/C2004A04997/2024-07-01/2024-07-01/text/1/epub/OEBPS/document_3/document_3.html#_Toc171751562"^^xsd:anyURI .

C2004A04997:233 a C2004A04997:Chapter ;
    rdfs:label "Chapter - C233 Chapter 49 Printed books newspapers pictures and other products of the printing industry manuscripts typescripts and plans"@en-AU ;
    dt:isPartOf C2004A04997:198 ;
    rdfs:comment "Chapter 49 Printed books newspapers pictures and other products of the printing industry manuscripts typescripts and plans - Abrievated Graph Key: C233"@en-AU ;
    skos:definition "Chapter 49 Printed books newspapers pictures and other products of the printing industry manuscripts typescripts and plans"@en-AU ;
    skos:narrower C2004A04997:198 ;
    skos:prefLabel "Chapter C233"@en-AU ;
    dcat:accessURL "https://www.legislation.gov.au/C2004A04997/2024-07-01/2024-07-01/text/1/epub/OEBPS/document_3/document_3.html#_Toc171751563"^^xsd:anyURI .

C2004A04997:234 a C2004A04997:Item ;
    rdfs:label "Item - I234 Notes"@en-AU ;
    dt:isPartOf C2004A04997:198 ;
    rdfs:comment "Notes - Abrievated Graph Key: I234"@en-AU ;
    skos:definition "Notes"@en-AU ;
    skos:narrower C2004A04997:198 ;
    skos:prefLabel "Item I234"@en-AU ;
    dcat:accessURL "https://www.legislation.gov.au/C2004A04997/2024-07-01/2024-07-01/text/1/epub/OEBPS/document_3/document_3.html#_Toc171751564"^^xsd:anyURI .

C2004A04997:235 a C2004A04997:Section ;
    rdfs:label "Section - S235 Section XITextiles and textile articles"@en-AU ;
    dt:isPartOf C2004A04997:198 ;
    rdfs:comment "Section XITextiles and textile articles - Abrievated Graph Key: S235"@en-AU ;
    skos:definition "Section XITextiles and textile articles"@en-AU ;
    skos:narrower C2004A04997:198 ;
    skos:prefLabel "Section S235"@en-AU ;
    dcat:accessURL "https://www.legislation.gov.au/C2004A04997/2024-07-01/2024-07-01/text/1/epub/OEBPS/document_3/document_3.html#_Toc171751565"^^xsd:anyURI .

C2004A04997:236 a C2004A04997:Item ;
    rdfs:label "Item - I236 Notes"@en-AU ;
    dt:isPartOf C2004A04997:198 ;
    rdfs:comment "Notes - Abrievated Graph Key: I236"@en-AU ;
    skos:definition "Notes"@en-AU ;
    skos:narrower C2004A04997:198 ;
    skos:prefLabel "Item I236"@en-AU ;
    dcat:accessURL "https://www.legislation.gov.au/C2004A04997/2024-07-01/2024-07-01/text/1/epub/OEBPS/document_3/document_3.html#_Toc171751566"^^xsd:anyURI .

C2004A04997:237 a C2004A04997:Item ;
    rdfs:label "Item - I237 Subheading Notes"@en-AU ;
    dt:isPartOf C2004A04997:198 ;
    rdfs:comment "Subheading Notes - Abrievated Graph Key: I237"@en-AU ;
    skos:definition "Subheading Notes"@en-AU ;
    skos:narrower C2004A04997:198 ;
    skos:prefLabel "Item I237"@en-AU ;
    dcat:accessURL "https://www.legislation.gov.au/C2004A04997/2024-07-01/2024-07-01/text/1/epub/OEBPS/document_3/document_3.html#_Toc171751567"^^xsd:anyURI .

C2004A04997:238 a C2004A04997:Item ;
    rdfs:label "Item - I238 Additional Notes"@en-AU ;
    dt:isPartOf C2004A04997:198 ;
    rdfs:comment "Additional Notes - Abrievated Graph Key: I238"@en-AU ;
    skos:definition "Additional Notes"@en-AU ;
    skos:narrower C2004A04997:198 ;
    skos:prefLabel "Item I238"@en-AU ;
    dcat:accessURL "https://www.legislation.gov.au/C2004A04997/2024-07-01/2024-07-01/text/1/epub/OEBPS/document_3/document_3.html#_Toc171751568"^^xsd:anyURI .

C2004A04997:239 a C2004A04997:Chapter ;
    rdfs:label "Chapter - C239 Chapter 50 Silk"@en-AU ;
    dt:isPartOf C2004A04997:198 ;
    rdfs:comment "Chapter 50 Silk - Abrievated Graph Key: C239"@en-AU ;
    skos:definition "Chapter 50 Silk"@en-AU ;
    skos:narrower C2004A04997:198 ;
    skos:prefLabel "Chapter C239"@en-AU ;
    dcat:accessURL "https://www.legislation.gov.au/C2004A04997/2024-07-01/2024-07-01/text/1/epub/OEBPS/document_3/document_3.html#_Toc171751569"^^xsd:anyURI .

C2004A04997:24 a C2004A04997:Item ;
    rdfs:label "Item - I24 13 EA  When goods are Pacific Islands originating goods"@en-AU ;
    dt:isPartOf C2004A04997:2 ;
    rdfs:comment "13 EA  When goods are Pacific Islands originating goods - Abrievated Graph Key: I24"@en-AU ;
    skos:definition "13 EA  When goods are Pacific Islands originating goods"@en-AU ;
    skos:narrower C2004A04997:2 ;
    skos:prefLabel "Item I24"@en-AU ;
    dcat:accessURL "https://www.legislation.gov.au/C2004A04997/2024-07-01/2024-07-01/text/1/epub/OEBPS/document_1/document_1.html#_Toc172806524"^^xsd:anyURI .

C2004A04997:240 a C2004A04997:Chapter ;
    rdfs:label "Chapter - C240 Chapter 51 Wool fine or coarse animal hair horsehair yarn and woven fabric"@en-AU ;
    dt:isPartOf C2004A04997:198 ;
    rdfs:comment "Chapter 51 Wool fine or coarse animal hair horsehair yarn and woven fabric - Abrievated Graph Key: C240"@en-AU ;
    skos:definition "Chapter 51 Wool fine or coarse animal hair horsehair yarn and woven fabric"@en-AU ;
    skos:narrower C2004A04997:198 ;
    skos:prefLabel "Chapter C240"@en-AU ;
    dcat:accessURL "https://www.legislation.gov.au/C2004A04997/2024-07-01/2024-07-01/text/1/epub/OEBPS/document_3/document_3.html#_Toc171751570"^^xsd:anyURI .

C2004A04997:241 a C2004A04997:Item ;
    rdfs:label "Item - I241 Note"@en-AU ;
    dt:isPartOf C2004A04997:198 ;
    rdfs:comment "Note - Abrievated Graph Key: I241"@en-AU ;
    skos:definition "Note"@en-AU ;
    skos:narrower C2004A04997:198 ;
    skos:prefLabel "Item I241"@en-AU ;
    dcat:accessURL "https://www.legislation.gov.au/C2004A04997/2024-07-01/2024-07-01/text/1/epub/OEBPS/document_3/document_3.html#_Toc171751571"^^xsd:anyURI .

C2004A04997:242 a C2004A04997:Chapter ;
    rdfs:label "Chapter - C242 Chapter 52 Cotton"@en-AU ;
    dt:isPartOf C2004A04997:198 ;
    rdfs:comment "Chapter 52 Cotton - Abrievated Graph Key: C242"@en-AU ;
    skos:definition "Chapter 52 Cotton"@en-AU ;
    skos:narrower C2004A04997:198 ;
    skos:prefLabel "Chapter C242"@en-AU ;
    dcat:accessURL "https://www.legislation.gov.au/C2004A04997/2024-07-01/2024-07-01/text/1/epub/OEBPS/document_3/document_3.html#_Toc171751572"^^xsd:anyURI .

C2004A04997:243 a C2004A04997:Item ;
    rdfs:label "Item - I243 Subheading Note"@en-AU ;
    dt:isPartOf C2004A04997:198 ;
    rdfs:comment "Subheading Note - Abrievated Graph Key: I243"@en-AU ;
    skos:definition "Subheading Note"@en-AU ;
    skos:narrower C2004A04997:198 ;
    skos:prefLabel "Item I243"@en-AU ;
    dcat:accessURL "https://www.legislation.gov.au/C2004A04997/2024-07-01/2024-07-01/text/1/epub/OEBPS/document_3/document_3.html#_Toc171751573"^^xsd:anyURI .

C2004A04997:244 a C2004A04997:Chapter ;
    rdfs:label "Chapter - C244 Chapter 53 Other vegetable textile fibres paper yarn and woven fabrics of paper yarn"@en-AU ;
    dt:isPartOf C2004A04997:198 ;
    rdfs:comment "Chapter 53 Other vegetable textile fibres paper yarn and woven fabrics of paper yarn - Abrievated Graph Key: C244"@en-AU ;
    skos:definition "Chapter 53 Other vegetable textile fibres paper yarn and woven fabrics of paper yarn"@en-AU ;
    skos:narrower C2004A04997:198 ;
    skos:prefLabel "Chapter C244"@en-AU ;
    dcat:accessURL "https://www.legislation.gov.au/C2004A04997/2024-07-01/2024-07-01/text/1/epub/OEBPS/document_3/document_3.html#_Toc171751574"^^xsd:anyURI .

C2004A04997:245 a C2004A04997:Chapter ;
    rdfs:label "Chapter - C245 Chapter 54 Man made filaments strip and the like of man made textile materials"@en-AU ;
    dt:isPartOf C2004A04997:198 ;
    rdfs:comment "Chapter 54 Man made filaments strip and the like of man made textile materials - Abrievated Graph Key: C245"@en-AU ;
    skos:definition "Chapter 54 Man made filaments strip and the like of man made textile materials"@en-AU ;
    skos:narrower C2004A04997:198 ;
    skos:prefLabel "Chapter C245"@en-AU ;
    dcat:accessURL "https://www.legislation.gov.au/C2004A04997/2024-07-01/2024-07-01/text/1/epub/OEBPS/document_3/document_3.html#_Toc171751575"^^xsd:anyURI .

C2004A04997:246 a C2004A04997:Item ;
    rdfs:label "Item - I246 Notes"@en-AU ;
    dt:isPartOf C2004A04997:198 ;
    rdfs:comment "Notes - Abrievated Graph Key: I246"@en-AU ;
    skos:definition "Notes"@en-AU ;
    skos:narrower C2004A04997:198 ;
    skos:prefLabel "Item I246"@en-AU ;
    dcat:accessURL "https://www.legislation.gov.au/C2004A04997/2024-07-01/2024-07-01/text/1/epub/OEBPS/document_3/document_3.html#_Toc171751576"^^xsd:anyURI .

C2004A04997:247 a C2004A04997:Chapter ;
    rdfs:label "Chapter - C247 Chapter 55 Man made staple fibres"@en-AU ;
    dt:isPartOf C2004A04997:198 ;
    rdfs:comment "Chapter 55 Man made staple fibres - Abrievated Graph Key: C247"@en-AU ;
    skos:definition "Chapter 55 Man made staple fibres"@en-AU ;
    skos:narrower C2004A04997:198 ;
    skos:prefLabel "Chapter C247"@en-AU ;
    dcat:accessURL "https://www.legislation.gov.au/C2004A04997/2024-07-01/2024-07-01/text/1/epub/OEBPS/document_3/document_3.html#_Toc171751577"^^xsd:anyURI .

C2004A04997:248 a C2004A04997:Item ;
    rdfs:label "Item - I248 Note"@en-AU ;
    dt:isPartOf C2004A04997:198 ;
    rdfs:comment "Note - Abrievated Graph Key: I248"@en-AU ;
    skos:definition "Note"@en-AU ;
    skos:narrower C2004A04997:198 ;
    skos:prefLabel "Item I248"@en-AU ;
    dcat:accessURL "https://www.legislation.gov.au/C2004A04997/2024-07-01/2024-07-01/text/1/epub/OEBPS/document_3/document_3.html#_Toc171751578"^^xsd:anyURI .

C2004A04997:249 a C2004A04997:Chapter ;
    rdfs:label "Chapter - C249 Chapter 56 Wadding felt and nonwovens special yarns twine cordage ropes and cables and articles thereof"@en-AU ;
    dt:isPartOf C2004A04997:198 ;
    rdfs:comment "Chapter 56 Wadding felt and nonwovens special yarns twine cordage ropes and cables and articles thereof - Abrievated Graph Key: C249"@en-AU ;
    skos:definition "Chapter 56 Wadding felt and nonwovens special yarns twine cordage ropes and cables and articles thereof"@en-AU ;
    skos:narrower C2004A04997:198 ;
    skos:prefLabel "Chapter C249"@en-AU ;
    dcat:accessURL "https://www.legislation.gov.au/C2004A04997/2024-07-01/2024-07-01/text/1/epub/OEBPS/document_3/document_3.html#_Toc171751579"^^xsd:anyURI .

C2004A04997:25 a C2004A04997:Item ;
    rdfs:label "Item - I25 13 EB  When goods are Trans Pacific Partnership originating goods"@en-AU ;
    dt:isPartOf C2004A04997:2 ;
    rdfs:comment "13 EB  When goods are Trans Pacific Partnership originating goods - Abrievated Graph Key: I25"@en-AU ;
    skos:definition "13 EB  When goods are Trans Pacific Partnership originating goods"@en-AU ;
    skos:narrower C2004A04997:2 ;
    skos:prefLabel "Item I25"@en-AU ;
    dcat:accessURL "https://www.legislation.gov.au/C2004A04997/2024-07-01/2024-07-01/text/1/epub/OEBPS/document_1/document_1.html#_Toc172806525"^^xsd:anyURI .

C2004A04997:250 a C2004A04997:Item ;
    rdfs:label "Item - I250 Notes"@en-AU ;
    dt:isPartOf C2004A04997:198 ;
    rdfs:comment "Notes - Abrievated Graph Key: I250"@en-AU ;
    skos:definition "Notes"@en-AU ;
    skos:narrower C2004A04997:198 ;
    skos:prefLabel "Item I250"@en-AU ;
    dcat:accessURL "https://www.legislation.gov.au/C2004A04997/2024-07-01/2024-07-01/text/1/epub/OEBPS/document_3/document_3.html#_Toc171751580"^^xsd:anyURI .

C2004A04997:251 a C2004A04997:Chapter ;
    rdfs:label "Chapter - C251 Chapter 57 Carpets and other textile floor coverings"@en-AU ;
    dt:isPartOf C2004A04997:198 ;
    rdfs:comment "Chapter 57 Carpets and other textile floor coverings - Abrievated Graph Key: C251"@en-AU ;
    skos:definition "Chapter 57 Carpets and other textile floor coverings"@en-AU ;
    skos:narrower C2004A04997:198 ;
    skos:prefLabel "Chapter C251"@en-AU ;
    dcat:accessURL "https://www.legislation.gov.au/C2004A04997/2024-07-01/2024-07-01/text/1/epub/OEBPS/document_3/document_3.html#_Toc171751581"^^xsd:anyURI .

C2004A04997:252 a C2004A04997:Item ;
    rdfs:label "Item - I252 Notes"@en-AU ;
    dt:isPartOf C2004A04997:198 ;
    rdfs:comment "Notes - Abrievated Graph Key: I252"@en-AU ;
    skos:definition "Notes"@en-AU ;
    skos:narrower C2004A04997:198 ;
    skos:prefLabel "Item I252"@en-AU ;
    dcat:accessURL "https://www.legislation.gov.au/C2004A04997/2024-07-01/2024-07-01/text/1/epub/OEBPS/document_3/document_3.html#_Toc171751582"^^xsd:anyURI .

C2004A04997:253 a C2004A04997:Item ;
    rdfs:label "Item - I253 Additional Notes"@en-AU ;
    dt:isPartOf C2004A04997:198 ;
    rdfs:comment "Additional Notes - Abrievated Graph Key: I253"@en-AU ;
    skos:definition "Additional Notes"@en-AU ;
    skos:narrower C2004A04997:198 ;
    skos:prefLabel "Item I253"@en-AU ;
    dcat:accessURL "https://www.legislation.gov.au/C2004A04997/2024-07-01/2024-07-01/text/1/epub/OEBPS/document_3/document_3.html#_Toc171751583"^^xsd:anyURI .

C2004A04997:254 a C2004A04997:Chapter ;
    rdfs:label "Chapter - C254 Chapter 58 Special woven fabrics tufted textile fabrics lace tapestries trimmings embroidery"@en-AU ;
    dt:isPartOf C2004A04997:198 ;
    rdfs:comment "Chapter 58 Special woven fabrics tufted textile fabrics lace tapestries trimmings embroidery - Abrievated Graph Key: C254"@en-AU ;
    skos:definition "Chapter 58 Special woven fabrics tufted textile fabrics lace tapestries trimmings embroidery"@en-AU ;
    skos:narrower C2004A04997:198 ;
    skos:prefLabel "Chapter C254"@en-AU ;
    dcat:accessURL "https://www.legislation.gov.au/C2004A04997/2024-07-01/2024-07-01/text/1/epub/OEBPS/document_3/document_3.html#_Toc171751584"^^xsd:anyURI .

C2004A04997:255 a C2004A04997:Item ;
    rdfs:label "Item - I255 Notes"@en-AU ;
    dt:isPartOf C2004A04997:198 ;
    rdfs:comment "Notes - Abrievated Graph Key: I255"@en-AU ;
    skos:definition "Notes"@en-AU ;
    skos:narrower C2004A04997:198 ;
    skos:prefLabel "Item I255"@en-AU ;
    dcat:accessURL "https://www.legislation.gov.au/C2004A04997/2024-07-01/2024-07-01/text/1/epub/OEBPS/document_3/document_3.html#_Toc171751585"^^xsd:anyURI .

C2004A04997:256 a C2004A04997:Item ;
    rdfs:label "Item - I256 Additional Note"@en-AU ;
    dt:isPartOf C2004A04997:198 ;
    rdfs:comment "Additional Note - Abrievated Graph Key: I256"@en-AU ;
    skos:definition "Additional Note"@en-AU ;
    skos:narrower C2004A04997:198 ;
    skos:prefLabel "Item I256"@en-AU ;
    dcat:accessURL "https://www.legislation.gov.au/C2004A04997/2024-07-01/2024-07-01/text/1/epub/OEBPS/document_3/document_3.html#_Toc171751586"^^xsd:anyURI .

C2004A04997:257 a C2004A04997:Chapter ;
    rdfs:label "Chapter - C257 Chapter 59 Impregnated coated covered or laminated textile fabrics textile articles of a kind suitable for industrial use"@en-AU ;
    dt:isPartOf C2004A04997:198 ;
    rdfs:comment "Chapter 59 Impregnated coated covered or laminated textile fabrics textile articles of a kind suitable for industrial use - Abrievated Graph Key: C257"@en-AU ;
    skos:definition "Chapter 59 Impregnated coated covered or laminated textile fabrics textile articles of a kind suitable for industrial use"@en-AU ;
    skos:narrower C2004A04997:198 ;
    skos:prefLabel "Chapter C257"@en-AU ;
    dcat:accessURL "https://www.legislation.gov.au/C2004A04997/2024-07-01/2024-07-01/text/1/epub/OEBPS/document_3/document_3.html#_Toc171751587"^^xsd:anyURI .

C2004A04997:258 a C2004A04997:Item ;
    rdfs:label "Item - I258 Notes"@en-AU ;
    dt:isPartOf C2004A04997:198 ;
    rdfs:comment "Notes - Abrievated Graph Key: I258"@en-AU ;
    skos:definition "Notes"@en-AU ;
    skos:narrower C2004A04997:198 ;
    skos:prefLabel "Item I258"@en-AU ;
    dcat:accessURL "https://www.legislation.gov.au/C2004A04997/2024-07-01/2024-07-01/text/1/epub/OEBPS/document_3/document_3.html#_Toc171751588"^^xsd:anyURI .

C2004A04997:26 a C2004A04997:Item ;
    rdfs:label "Item - I26 13 F  When goods are Malaysian originating goods"@en-AU ;
    dt:isPartOf C2004A04997:2 ;
    rdfs:comment "13 F  When goods are Malaysian originating goods - Abrievated Graph Key: I26"@en-AU ;
    skos:definition "13 F  When goods are Malaysian originating goods"@en-AU ;
    skos:narrower C2004A04997:2 ;
    skos:prefLabel "Item I26"@en-AU ;
    dcat:accessURL "https://www.legislation.gov.au/C2004A04997/2024-07-01/2024-07-01/text/1/epub/OEBPS/document_1/document_1.html#_Toc172806526"^^xsd:anyURI .

C2004A04997:260 a C2004A04997:Schedule ;
    rdfs:label "Schedule - S260 Schedule 3 Classification of goods and general and special rates of duty"@en-AU ;
    dt:isPartOf C2004A04997:259 ;
    rdfs:comment "Schedule 3 Classification of goods and general and special rates of duty - Abrievated Graph Key: S260"@en-AU ;
    skos:definition "Schedule 3 Classification of goods and general and special rates of duty"@en-AU ;
    skos:narrower C2004A04997:259 ;
    skos:prefLabel "Schedule S260"@en-AU ;
    dcat:accessURL "https://www.legislation.gov.au/C2004A04997/2024-07-01/2024-07-01/text/1/epub/OEBPS/document_4/document_4.html#_Toc171751991"^^xsd:anyURI .

C2004A04997:262 a C2004A04997:Chapter ;
    rdfs:label "Chapter - C262 Chapter 60 Knitted or crocheted fabrics"@en-AU ;
    dt:isPartOf C2004A04997:261 ;
    rdfs:comment "Chapter 60 Knitted or crocheted fabrics - Abrievated Graph Key: C262"@en-AU ;
    skos:definition "Chapter 60 Knitted or crocheted fabrics"@en-AU ;
    skos:narrower C2004A04997:261 ;
    skos:prefLabel "Chapter C262"@en-AU ;
    dcat:accessURL "https://www.legislation.gov.au/C2004A04997/2024-07-01/2024-07-01/text/1/epub/OEBPS/document_4/document_4.html#_Toc171751993"^^xsd:anyURI .

C2004A04997:263 a C2004A04997:Item ;
    rdfs:label "Item - I263 Notes"@en-AU ;
    dt:isPartOf C2004A04997:261 ;
    rdfs:comment "Notes - Abrievated Graph Key: I263"@en-AU ;
    skos:definition "Notes"@en-AU ;
    skos:narrower C2004A04997:261 ;
    skos:prefLabel "Item I263"@en-AU ;
    dcat:accessURL "https://www.legislation.gov.au/C2004A04997/2024-07-01/2024-07-01/text/1/epub/OEBPS/document_4/document_4.html#_Toc171751994"^^xsd:anyURI .

C2004A04997:264 a C2004A04997:Item ;
    rdfs:label "Item - I264 Subheading Note"@en-AU ;
    dt:isPartOf C2004A04997:261 ;
    rdfs:comment "Subheading Note - Abrievated Graph Key: I264"@en-AU ;
    skos:definition "Subheading Note"@en-AU ;
    skos:narrower C2004A04997:261 ;
    skos:prefLabel "Item I264"@en-AU ;
    dcat:accessURL "https://www.legislation.gov.au/C2004A04997/2024-07-01/2024-07-01/text/1/epub/OEBPS/document_4/document_4.html#_Toc171751995"^^xsd:anyURI .

C2004A04997:265 a C2004A04997:Chapter ;
    rdfs:label "Chapter - C265 Chapter 61 Articles of apparel and clothing accessories knitted or crocheted"@en-AU ;
    dt:isPartOf C2004A04997:261 ;
    rdfs:comment "Chapter 61 Articles of apparel and clothing accessories knitted or crocheted - Abrievated Graph Key: C265"@en-AU ;
    skos:definition "Chapter 61 Articles of apparel and clothing accessories knitted or crocheted"@en-AU ;
    skos:narrower C2004A04997:261 ;
    skos:prefLabel "Chapter C265"@en-AU ;
    dcat:accessURL "https://www.legislation.gov.au/C2004A04997/2024-07-01/2024-07-01/text/1/epub/OEBPS/document_4/document_4.html#_Toc171751996"^^xsd:anyURI .

C2004A04997:266 a C2004A04997:Item ;
    rdfs:label "Item - I266 Notes"@en-AU ;
    dt:isPartOf C2004A04997:261 ;
    rdfs:comment "Notes - Abrievated Graph Key: I266"@en-AU ;
    skos:definition "Notes"@en-AU ;
    skos:narrower C2004A04997:261 ;
    skos:prefLabel "Item I266"@en-AU ;
    dcat:accessURL "https://www.legislation.gov.au/C2004A04997/2024-07-01/2024-07-01/text/1/epub/OEBPS/document_4/document_4.html#_Toc171751997"^^xsd:anyURI .

C2004A04997:267 a C2004A04997:Item ;
    rdfs:label "Item - I267 Additional Note"@en-AU ;
    dt:isPartOf C2004A04997:261 ;
    rdfs:comment "Additional Note - Abrievated Graph Key: I267"@en-AU ;
    skos:definition "Additional Note"@en-AU ;
    skos:narrower C2004A04997:261 ;
    skos:prefLabel "Item I267"@en-AU ;
    dcat:accessURL "https://www.legislation.gov.au/C2004A04997/2024-07-01/2024-07-01/text/1/epub/OEBPS/document_4/document_4.html#_Toc171751998"^^xsd:anyURI .

C2004A04997:268 a C2004A04997:Chapter ;
    rdfs:label "Chapter - C268 Chapter 62 Articles of apparel and clothing accessories not knitted or crocheted"@en-AU ;
    dt:isPartOf C2004A04997:261 ;
    rdfs:comment "Chapter 62 Articles of apparel and clothing accessories not knitted or crocheted - Abrievated Graph Key: C268"@en-AU ;
    skos:definition "Chapter 62 Articles of apparel and clothing accessories not knitted or crocheted"@en-AU ;
    skos:narrower C2004A04997:261 ;
    skos:prefLabel "Chapter C268"@en-AU ;
    dcat:accessURL "https://www.legislation.gov.au/C2004A04997/2024-07-01/2024-07-01/text/1/epub/OEBPS/document_4/document_4.html#_Toc171751999"^^xsd:anyURI .

C2004A04997:269 a C2004A04997:Item ;
    rdfs:label "Item - I269 Notes"@en-AU ;
    dt:isPartOf C2004A04997:261 ;
    rdfs:comment "Notes - Abrievated Graph Key: I269"@en-AU ;
    skos:definition "Notes"@en-AU ;
    skos:narrower C2004A04997:261 ;
    skos:prefLabel "Item I269"@en-AU ;
    dcat:accessURL "https://www.legislation.gov.au/C2004A04997/2024-07-01/2024-07-01/text/1/epub/OEBPS/document_4/document_4.html#_Toc171752000"^^xsd:anyURI .

C2004A04997:27 a C2004A04997:Item ;
    rdfs:label "Item - I27 13 FA  When goods are Indonesian originating goods"@en-AU ;
    dt:isPartOf C2004A04997:2 ;
    rdfs:comment "13 FA  When goods are Indonesian originating goods - Abrievated Graph Key: I27"@en-AU ;
    skos:definition "13 FA  When goods are Indonesian originating goods"@en-AU ;
    skos:narrower C2004A04997:2 ;
    skos:prefLabel "Item I27"@en-AU ;
    dcat:accessURL "https://www.legislation.gov.au/C2004A04997/2024-07-01/2024-07-01/text/1/epub/OEBPS/document_1/document_1.html#_Toc172806527"^^xsd:anyURI .

C2004A04997:270 a C2004A04997:Item ;
    rdfs:label "Item - I270 Additional Note"@en-AU ;
    dt:isPartOf C2004A04997:261 ;
    rdfs:comment "Additional Note - Abrievated Graph Key: I270"@en-AU ;
    skos:definition "Additional Note"@en-AU ;
    skos:narrower C2004A04997:261 ;
    skos:prefLabel "Item I270"@en-AU ;
    dcat:accessURL "https://www.legislation.gov.au/C2004A04997/2024-07-01/2024-07-01/text/1/epub/OEBPS/document_4/document_4.html#_Toc171752001"^^xsd:anyURI .

C2004A04997:271 a C2004A04997:Chapter ;
    rdfs:label "Chapter - C271 Chapter 63 Other made up textile articles sets worn clothing and worn textile articles rags"@en-AU ;
    dt:isPartOf C2004A04997:261 ;
    rdfs:comment "Chapter 63 Other made up textile articles sets worn clothing and worn textile articles rags - Abrievated Graph Key: C271"@en-AU ;
    skos:definition "Chapter 63 Other made up textile articles sets worn clothing and worn textile articles rags"@en-AU ;
    skos:narrower C2004A04997:261 ;
    skos:prefLabel "Chapter C271"@en-AU ;
    dcat:accessURL "https://www.legislation.gov.au/C2004A04997/2024-07-01/2024-07-01/text/1/epub/OEBPS/document_4/document_4.html#_Toc171752002"^^xsd:anyURI .

C2004A04997:272 a C2004A04997:Item ;
    rdfs:label "Item - I272 Notes"@en-AU ;
    dt:isPartOf C2004A04997:261 ;
    rdfs:comment "Notes - Abrievated Graph Key: I272"@en-AU ;
    skos:definition "Notes"@en-AU ;
    skos:narrower C2004A04997:261 ;
    skos:prefLabel "Item I272"@en-AU ;
    dcat:accessURL "https://www.legislation.gov.au/C2004A04997/2024-07-01/2024-07-01/text/1/epub/OEBPS/document_4/document_4.html#_Toc171752003"^^xsd:anyURI .

C2004A04997:273 a C2004A04997:Item ;
    rdfs:label "Item - I273 Subheading Note"@en-AU ;
    dt:isPartOf C2004A04997:261 ;
    rdfs:comment "Subheading Note - Abrievated Graph Key: I273"@en-AU ;
    skos:definition "Subheading Note"@en-AU ;
    skos:narrower C2004A04997:261 ;
    skos:prefLabel "Item I273"@en-AU ;
    dcat:accessURL "https://www.legislation.gov.au/C2004A04997/2024-07-01/2024-07-01/text/1/epub/OEBPS/document_4/document_4.html#_Toc171752004"^^xsd:anyURI .

C2004A04997:274 a C2004A04997:Item ;
    rdfs:label "Item - I274 Sub Chapter IOther made up textile articles"@en-AU ;
    dt:isPartOf C2004A04997:261 ;
    rdfs:comment "Sub Chapter IOther made up textile articles - Abrievated Graph Key: I274"@en-AU ;
    skos:definition "Sub Chapter IOther made up textile articles"@en-AU ;
    skos:narrower C2004A04997:261 ;
    skos:prefLabel "Item I274"@en-AU ;
    dcat:accessURL "https://www.legislation.gov.au/C2004A04997/2024-07-01/2024-07-01/text/1/epub/OEBPS/document_4/document_4.html#_Toc171752005"^^xsd:anyURI .

C2004A04997:275 a C2004A04997:Item ;
    rdfs:label "Item - I275 Sub Chapter IISets"@en-AU ;
    dt:isPartOf C2004A04997:261 ;
    rdfs:comment "Sub Chapter IISets - Abrievated Graph Key: I275"@en-AU ;
    skos:definition "Sub Chapter IISets"@en-AU ;
    skos:narrower C2004A04997:261 ;
    skos:prefLabel "Item I275"@en-AU ;
    dcat:accessURL "https://www.legislation.gov.au/C2004A04997/2024-07-01/2024-07-01/text/1/epub/OEBPS/document_4/document_4.html#_Toc171752006"^^xsd:anyURI .

C2004A04997:276 a C2004A04997:Item ;
    rdfs:label "Item - I276 Sub Chapter IIIWorn clothing and worn textile articles rags"@en-AU ;
    dt:isPartOf C2004A04997:261 ;
    rdfs:comment "Sub Chapter IIIWorn clothing and worn textile articles rags - Abrievated Graph Key: I276"@en-AU ;
    skos:definition "Sub Chapter IIIWorn clothing and worn textile articles rags"@en-AU ;
    skos:narrower C2004A04997:261 ;
    skos:prefLabel "Item I276"@en-AU ;
    dcat:accessURL "https://www.legislation.gov.au/C2004A04997/2024-07-01/2024-07-01/text/1/epub/OEBPS/document_4/document_4.html#_Toc171752007"^^xsd:anyURI .

C2004A04997:279 a C2004A04997:Item ;
    rdfs:label "Item - I279 Notes"@en-AU ;
    dt:isPartOf C2004A04997:278 ;
    rdfs:comment "Notes - Abrievated Graph Key: I279"@en-AU ;
    skos:definition "Notes"@en-AU ;
    skos:narrower C2004A04997:278 ;
    skos:prefLabel "Item I279"@en-AU ;
    dcat:accessURL "https://www.legislation.gov.au/C2004A04997/2024-07-01/2024-07-01/text/1/epub/OEBPS/document_4/document_4.html#_Toc171752010"^^xsd:anyURI .

C2004A04997:28 a C2004A04997:Item ;
    rdfs:label "Item - I28 13 G  When goods are Korean originating goods"@en-AU ;
    dt:isPartOf C2004A04997:2 ;
    rdfs:comment "13 G  When goods are Korean originating goods - Abrievated Graph Key: I28"@en-AU ;
    skos:definition "13 G  When goods are Korean originating goods"@en-AU ;
    skos:narrower C2004A04997:2 ;
    skos:prefLabel "Item I28"@en-AU ;
    dcat:accessURL "https://www.legislation.gov.au/C2004A04997/2024-07-01/2024-07-01/text/1/epub/OEBPS/document_1/document_1.html#_Toc172806528"^^xsd:anyURI .

C2004A04997:280 a C2004A04997:Item ;
    rdfs:label "Item - I280 Subheading Note"@en-AU ;
    dt:isPartOf C2004A04997:278 ;
    rdfs:comment "Subheading Note - Abrievated Graph Key: I280"@en-AU ;
    skos:definition "Subheading Note"@en-AU ;
    skos:narrower C2004A04997:278 ;
    skos:prefLabel "Item I280"@en-AU ;
    dcat:accessURL "https://www.legislation.gov.au/C2004A04997/2024-07-01/2024-07-01/text/1/epub/OEBPS/document_4/document_4.html#_Toc171752011"^^xsd:anyURI .

C2004A04997:282 a C2004A04997:Item ;
    rdfs:label "Item - I282 Notes"@en-AU ;
    dt:isPartOf C2004A04997:281 ;
    rdfs:comment "Notes - Abrievated Graph Key: I282"@en-AU ;
    skos:definition "Notes"@en-AU ;
    skos:narrower C2004A04997:281 ;
    skos:prefLabel "Item I282"@en-AU ;
    dcat:accessURL "https://www.legislation.gov.au/C2004A04997/2024-07-01/2024-07-01/text/1/epub/OEBPS/document_4/document_4.html#_Toc171752013"^^xsd:anyURI .

C2004A04997:284 a C2004A04997:Item ;
    rdfs:label "Item - I284 Notes"@en-AU ;
    dt:isPartOf C2004A04997:283 ;
    rdfs:comment "Notes - Abrievated Graph Key: I284"@en-AU ;
    skos:definition "Notes"@en-AU ;
    skos:narrower C2004A04997:283 ;
    skos:prefLabel "Item I284"@en-AU ;
    dcat:accessURL "https://www.legislation.gov.au/C2004A04997/2024-07-01/2024-07-01/text/1/epub/OEBPS/document_4/document_4.html#_Toc171752015"^^xsd:anyURI .

C2004A04997:286 a C2004A04997:Item ;
    rdfs:label "Item - I286 Notes"@en-AU ;
    dt:isPartOf C2004A04997:285 ;
    rdfs:comment "Notes - Abrievated Graph Key: I286"@en-AU ;
    skos:definition "Notes"@en-AU ;
    skos:narrower C2004A04997:285 ;
    skos:prefLabel "Item I286"@en-AU ;
    dcat:accessURL "https://www.legislation.gov.au/C2004A04997/2024-07-01/2024-07-01/text/1/epub/OEBPS/document_4/document_4.html#_Toc171752017"^^xsd:anyURI .

C2004A04997:289 a C2004A04997:Item ;
    rdfs:label "Item - I289 Notes"@en-AU ;
    dt:isPartOf C2004A04997:288 ;
    rdfs:comment "Notes - Abrievated Graph Key: I289"@en-AU ;
    skos:definition "Notes"@en-AU ;
    skos:narrower C2004A04997:288 ;
    skos:prefLabel "Item I289"@en-AU ;
    dcat:accessURL "https://www.legislation.gov.au/C2004A04997/2024-07-01/2024-07-01/text/1/epub/OEBPS/document_4/document_4.html#_Toc171752020"^^xsd:anyURI .

C2004A04997:29 a C2004A04997:Item ;
    rdfs:label "Item - I29 13 GA  When goods are Indian originating goods"@en-AU ;
    dt:isPartOf C2004A04997:2 ;
    rdfs:comment "13 GA  When goods are Indian originating goods - Abrievated Graph Key: I29"@en-AU ;
    skos:definition "13 GA  When goods are Indian originating goods"@en-AU ;
    skos:narrower C2004A04997:2 ;
    skos:prefLabel "Item I29"@en-AU ;
    dcat:accessURL "https://www.legislation.gov.au/C2004A04997/2024-07-01/2024-07-01/text/1/epub/OEBPS/document_1/document_1.html#_Toc172806529"^^xsd:anyURI .

C2004A04997:291 a C2004A04997:Item ;
    rdfs:label "Item - I291 Notes"@en-AU ;
    dt:isPartOf C2004A04997:290 ;
    rdfs:comment "Notes - Abrievated Graph Key: I291"@en-AU ;
    skos:definition "Notes"@en-AU ;
    skos:narrower C2004A04997:290 ;
    skos:prefLabel "Item I291"@en-AU ;
    dcat:accessURL "https://www.legislation.gov.au/C2004A04997/2024-07-01/2024-07-01/text/1/epub/OEBPS/document_4/document_4.html#_Toc171752022"^^xsd:anyURI .

C2004A04997:292 a C2004A04997:Item ;
    rdfs:label "Item - I292 Sub Chapter IGoods of siliceous fossil meals or of similar siliceous earths and refractory goods"@en-AU ;
    dt:isPartOf C2004A04997:290 ;
    rdfs:comment "Sub Chapter IGoods of siliceous fossil meals or of similar siliceous earths and refractory goods - Abrievated Graph Key: I292"@en-AU ;
    skos:definition "Sub Chapter IGoods of siliceous fossil meals or of similar siliceous earths and refractory goods"@en-AU ;
    skos:narrower C2004A04997:290 ;
    skos:prefLabel "Item I292"@en-AU ;
    dcat:accessURL "https://www.legislation.gov.au/C2004A04997/2024-07-01/2024-07-01/text/1/epub/OEBPS/document_4/document_4.html#_Toc171752023"^^xsd:anyURI .

C2004A04997:293 a C2004A04997:Item ;
    rdfs:label "Item - I293 Sub Chapter IIOther ceramic products"@en-AU ;
    dt:isPartOf C2004A04997:290 ;
    rdfs:comment "Sub Chapter IIOther ceramic products - Abrievated Graph Key: I293"@en-AU ;
    skos:definition "Sub Chapter IIOther ceramic products"@en-AU ;
    skos:narrower C2004A04997:290 ;
    skos:prefLabel "Item I293"@en-AU ;
    dcat:accessURL "https://www.legislation.gov.au/C2004A04997/2024-07-01/2024-07-01/text/1/epub/OEBPS/document_4/document_4.html#_Toc171752024"^^xsd:anyURI .

C2004A04997:295 a C2004A04997:Item ;
    rdfs:label "Item - I295 Notes"@en-AU ;
    dt:isPartOf C2004A04997:294 ;
    rdfs:comment "Notes - Abrievated Graph Key: I295"@en-AU ;
    skos:definition "Notes"@en-AU ;
    skos:narrower C2004A04997:294 ;
    skos:prefLabel "Item I295"@en-AU ;
    dcat:accessURL "https://www.legislation.gov.au/C2004A04997/2024-07-01/2024-07-01/text/1/epub/OEBPS/document_4/document_4.html#_Toc171752026"^^xsd:anyURI .

C2004A04997:296 a C2004A04997:Item ;
    rdfs:label "Item - I296 Subheading Note"@en-AU ;
    dt:isPartOf C2004A04997:294 ;
    rdfs:comment "Subheading Note - Abrievated Graph Key: I296"@en-AU ;
    skos:definition "Subheading Note"@en-AU ;
    skos:narrower C2004A04997:294 ;
    skos:prefLabel "Item I296"@en-AU ;
    dcat:accessURL "https://www.legislation.gov.au/C2004A04997/2024-07-01/2024-07-01/text/1/epub/OEBPS/document_4/document_4.html#_Toc171752027"^^xsd:anyURI .

C2004A04997:299 a C2004A04997:Item ;
    rdfs:label "Item - I299 Notes"@en-AU ;
    dt:isPartOf C2004A04997:298 ;
    rdfs:comment "Notes - Abrievated Graph Key: I299"@en-AU ;
    skos:definition "Notes"@en-AU ;
    skos:narrower C2004A04997:298 ;
    skos:prefLabel "Item I299"@en-AU ;
    dcat:accessURL "https://www.legislation.gov.au/C2004A04997/2024-07-01/2024-07-01/text/1/epub/OEBPS/document_4/document_4.html#_Toc171752030"^^xsd:anyURI .

C2004A04997:3 a C2004A04997:Item ;
    rdfs:label "Item - I3 1  Short title"@en-AU ;
    dt:isPartOf C2004A04997:2 ;
    rdfs:comment "1  Short title - Abrievated Graph Key: I3"@en-AU ;
    skos:definition "1  Short title"@en-AU ;
    skos:narrower C2004A04997:2 ;
    skos:prefLabel "Item I3"@en-AU ;
    dcat:accessURL "https://www.legislation.gov.au/C2004A04997/2024-07-01/2024-07-01/text/1/epub/OEBPS/document_1/document_1.html#_Toc172806503"^^xsd:anyURI .

C2004A04997:30 a C2004A04997:Item ;
    rdfs:label "Item - I30 13 H  When goods are Japanese originating goods"@en-AU ;
    dt:isPartOf C2004A04997:2 ;
    rdfs:comment "13 H  When goods are Japanese originating goods - Abrievated Graph Key: I30"@en-AU ;
    skos:definition "13 H  When goods are Japanese originating goods"@en-AU ;
    skos:narrower C2004A04997:2 ;
    skos:prefLabel "Item I30"@en-AU ;
    dcat:accessURL "https://www.legislation.gov.au/C2004A04997/2024-07-01/2024-07-01/text/1/epub/OEBPS/document_1/document_1.html#_Toc172806530"^^xsd:anyURI .

C2004A04997:300 a C2004A04997:Item ;
    rdfs:label "Item - I300 Subheading Notes"@en-AU ;
    dt:isPartOf C2004A04997:298 ;
    rdfs:comment "Subheading Notes - Abrievated Graph Key: I300"@en-AU ;
    skos:definition "Subheading Notes"@en-AU ;
    skos:narrower C2004A04997:298 ;
    skos:prefLabel "Item I300"@en-AU ;
    dcat:accessURL "https://www.legislation.gov.au/C2004A04997/2024-07-01/2024-07-01/text/1/epub/OEBPS/document_4/document_4.html#_Toc171752031"^^xsd:anyURI .

C2004A04997:301 a C2004A04997:Item ;
    rdfs:label "Item - I301 Sub Chapter INatural or cultured pearls and precious or semi precious stones"@en-AU ;
    dt:isPartOf C2004A04997:298 ;
    rdfs:comment "Sub Chapter INatural or cultured pearls and precious or semi precious stones - Abrievated Graph Key: I301"@en-AU ;
    skos:definition "Sub Chapter INatural or cultured pearls and precious or semi precious stones"@en-AU ;
    skos:narrower C2004A04997:298 ;
    skos:prefLabel "Item I301"@en-AU ;
    dcat:accessURL "https://www.legislation.gov.au/C2004A04997/2024-07-01/2024-07-01/text/1/epub/OEBPS/document_4/document_4.html#_Toc171752032"^^xsd:anyURI .

C2004A04997:302 a C2004A04997:Item ;
    rdfs:label "Item - I302 Sub Chapter IIPrecious metals and metals clad with precious metal"@en-AU ;
    dt:isPartOf C2004A04997:298 ;
    rdfs:comment "Sub Chapter IIPrecious metals and metals clad with precious metal - Abrievated Graph Key: I302"@en-AU ;
    skos:definition "Sub Chapter IIPrecious metals and metals clad with precious metal"@en-AU ;
    skos:narrower C2004A04997:298 ;
    skos:prefLabel "Item I302"@en-AU ;
    dcat:accessURL "https://www.legislation.gov.au/C2004A04997/2024-07-01/2024-07-01/text/1/epub/OEBPS/document_4/document_4.html#_Toc171752033"^^xsd:anyURI .

C2004A04997:303 a C2004A04997:Item ;
    rdfs:label "Item - I303 Sub Chapter IIIJewellery goldsmiths and silversmiths wares and other articles"@en-AU ;
    dt:isPartOf C2004A04997:298 ;
    rdfs:comment "Sub Chapter IIIJewellery goldsmiths and silversmiths wares and other articles - Abrievated Graph Key: I303"@en-AU ;
    skos:definition "Sub Chapter IIIJewellery goldsmiths and silversmiths wares and other articles"@en-AU ;
    skos:narrower C2004A04997:298 ;
    skos:prefLabel "Item I303"@en-AU ;
    dcat:accessURL "https://www.legislation.gov.au/C2004A04997/2024-07-01/2024-07-01/text/1/epub/OEBPS/document_4/document_4.html#_Toc171752034"^^xsd:anyURI .

C2004A04997:305 a C2004A04997:Item ;
    rdfs:label "Item - I305 Notes"@en-AU ;
    dt:isPartOf C2004A04997:304 ;
    rdfs:comment "Notes - Abrievated Graph Key: I305"@en-AU ;
    skos:definition "Notes"@en-AU ;
    skos:narrower C2004A04997:304 ;
    skos:prefLabel "Item I305"@en-AU ;
    dcat:accessURL "https://www.legislation.gov.au/C2004A04997/2024-07-01/2024-07-01/text/1/epub/OEBPS/document_4/document_4.html#_Toc171752036"^^xsd:anyURI .

C2004A04997:307 a C2004A04997:Item ;
    rdfs:label "Item - I307 Notes"@en-AU ;
    dt:isPartOf C2004A04997:306 ;
    rdfs:comment "Notes - Abrievated Graph Key: I307"@en-AU ;
    skos:definition "Notes"@en-AU ;
    skos:narrower C2004A04997:306 ;
    skos:prefLabel "Item I307"@en-AU ;
    dcat:accessURL "https://www.legislation.gov.au/C2004A04997/2024-07-01/2024-07-01/text/1/epub/OEBPS/document_4/document_4.html#_Toc171752038"^^xsd:anyURI .

C2004A04997:308 a C2004A04997:Item ;
    rdfs:label "Item - I308 Subheading Notes"@en-AU ;
    dt:isPartOf C2004A04997:306 ;
    rdfs:comment "Subheading Notes - Abrievated Graph Key: I308"@en-AU ;
    skos:definition "Subheading Notes"@en-AU ;
    skos:narrower C2004A04997:306 ;
    skos:prefLabel "Item I308"@en-AU ;
    dcat:accessURL "https://www.legislation.gov.au/C2004A04997/2024-07-01/2024-07-01/text/1/epub/OEBPS/document_4/document_4.html#_Toc171752039"^^xsd:anyURI .

C2004A04997:309 a C2004A04997:Item ;
    rdfs:label "Item - I309 Additional Note"@en-AU ;
    dt:isPartOf C2004A04997:306 ;
    rdfs:comment "Additional Note - Abrievated Graph Key: I309"@en-AU ;
    skos:definition "Additional Note"@en-AU ;
    skos:narrower C2004A04997:306 ;
    skos:prefLabel "Item I309"@en-AU ;
    dcat:accessURL "https://www.legislation.gov.au/C2004A04997/2024-07-01/2024-07-01/text/1/epub/OEBPS/document_4/document_4.html#_Toc171752040"^^xsd:anyURI .

C2004A04997:31 a C2004A04997:Item ;
    rdfs:label "Item - I31 13 J  When goods are Chinese originating goods"@en-AU ;
    dt:isPartOf C2004A04997:2 ;
    rdfs:comment "13 J  When goods are Chinese originating goods - Abrievated Graph Key: I31"@en-AU ;
    skos:definition "13 J  When goods are Chinese originating goods"@en-AU ;
    skos:narrower C2004A04997:2 ;
    skos:prefLabel "Item I31"@en-AU ;
    dcat:accessURL "https://www.legislation.gov.au/C2004A04997/2024-07-01/2024-07-01/text/1/epub/OEBPS/document_1/document_1.html#_Toc172806531"^^xsd:anyURI .

C2004A04997:310 a C2004A04997:Item ;
    rdfs:label "Item - I310 Sub Chapter IPrimary materials products in granular or powder form"@en-AU ;
    dt:isPartOf C2004A04997:306 ;
    rdfs:comment "Sub Chapter IPrimary materials products in granular or powder form - Abrievated Graph Key: I310"@en-AU ;
    skos:definition "Sub Chapter IPrimary materials products in granular or powder form"@en-AU ;
    skos:narrower C2004A04997:306 ;
    skos:prefLabel "Item I310"@en-AU ;
    dcat:accessURL "https://www.legislation.gov.au/C2004A04997/2024-07-01/2024-07-01/text/1/epub/OEBPS/document_4/document_4.html#_Toc171752041"^^xsd:anyURI .

C2004A04997:311 a C2004A04997:Item ;
    rdfs:label "Item - I311 Sub Chapter IIIron and non alloy steel"@en-AU ;
    dt:isPartOf C2004A04997:306 ;
    rdfs:comment "Sub Chapter IIIron and non alloy steel - Abrievated Graph Key: I311"@en-AU ;
    skos:definition "Sub Chapter IIIron and non alloy steel"@en-AU ;
    skos:narrower C2004A04997:306 ;
    skos:prefLabel "Item I311"@en-AU ;
    dcat:accessURL "https://www.legislation.gov.au/C2004A04997/2024-07-01/2024-07-01/text/1/epub/OEBPS/document_4/document_4.html#_Toc171752042"^^xsd:anyURI .

C2004A04997:312 a C2004A04997:Item ;
    rdfs:label "Item - I312 Sub Chapter IIIStainless steel"@en-AU ;
    dt:isPartOf C2004A04997:306 ;
    rdfs:comment "Sub Chapter IIIStainless steel - Abrievated Graph Key: I312"@en-AU ;
    skos:definition "Sub Chapter IIIStainless steel"@en-AU ;
    skos:narrower C2004A04997:306 ;
    skos:prefLabel "Item I312"@en-AU ;
    dcat:accessURL "https://www.legislation.gov.au/C2004A04997/2024-07-01/2024-07-01/text/1/epub/OEBPS/document_4/document_4.html#_Toc171752043"^^xsd:anyURI .

C2004A04997:313 a C2004A04997:Item ;
    rdfs:label "Item - I313 Sub Chapter IVOther alloy steel hollow drill bars and rods of alloy or non alloy steel"@en-AU ;
    dt:isPartOf C2004A04997:306 ;
    rdfs:comment "Sub Chapter IVOther alloy steel hollow drill bars and rods of alloy or non alloy steel - Abrievated Graph Key: I313"@en-AU ;
    skos:definition "Sub Chapter IVOther alloy steel hollow drill bars and rods of alloy or non alloy steel"@en-AU ;
    skos:narrower C2004A04997:306 ;
    skos:prefLabel "Item I313"@en-AU ;
    dcat:accessURL "https://www.legislation.gov.au/C2004A04997/2024-07-01/2024-07-01/text/1/epub/OEBPS/document_4/document_4.html#_Toc171752044"^^xsd:anyURI .

C2004A04997:315 a C2004A04997:Item ;
    rdfs:label "Item - I315 Notes"@en-AU ;
    dt:isPartOf C2004A04997:314 ;
    rdfs:comment "Notes - Abrievated Graph Key: I315"@en-AU ;
    skos:definition "Notes"@en-AU ;
    skos:narrower C2004A04997:314 ;
    skos:prefLabel "Item I315"@en-AU ;
    dcat:accessURL "https://www.legislation.gov.au/C2004A04997/2024-07-01/2024-07-01/text/1/epub/OEBPS/document_4/document_4.html#_Toc171752046"^^xsd:anyURI .

C2004A04997:316 a C2004A04997:Item ;
    rdfs:label "Item - I316 Additional Notes"@en-AU ;
    dt:isPartOf C2004A04997:314 ;
    rdfs:comment "Additional Notes - Abrievated Graph Key: I316"@en-AU ;
    skos:definition "Additional Notes"@en-AU ;
    skos:narrower C2004A04997:314 ;
    skos:prefLabel "Item I316"@en-AU ;
    dcat:accessURL "https://www.legislation.gov.au/C2004A04997/2024-07-01/2024-07-01/text/1/epub/OEBPS/document_4/document_4.html#_Toc171752047"^^xsd:anyURI .

C2004A04997:317 a C2004A04997:Volume ;
    rdfs:label "Volume - V317 Volume 5"@en-AU ;
    dt:hasPart C2004A04997:318 ;
    rdfs:comment "Volume 5 - Abrievated Graph Key: V317"@en-AU ;
    skos:broader C2004A04997:318 ;
    skos:definition "Volume 5"@en-AU ;
    skos:prefLabel "Volume V317"@en-AU ;
    dcat:accessURL "https://www.legislation.gov.au/C2004A04997/2024-07-01/2024-07-01/text/1/epub/OEBPS/document_5/document_5.html"^^xsd:anyURI .

C2004A04997:319 a C2004A04997:Section ;
    rdfs:label "Section - S319 Section XVBase metals and articles of base metal"@en-AU ;
    dt:isPartOf C2004A04997:318 ;
    rdfs:comment "Section XVBase metals and articles of base metal - Abrievated Graph Key: S319"@en-AU ;
    skos:definition "Section XVBase metals and articles of base metal"@en-AU ;
    skos:narrower C2004A04997:318 ;
    skos:prefLabel "Section S319"@en-AU ;
    dcat:accessURL "https://www.legislation.gov.au/C2004A04997/2024-07-01/2024-07-01/text/1/epub/OEBPS/document_5/document_5.html#_Toc171753161"^^xsd:anyURI .

C2004A04997:32 a C2004A04997:Item ;
    rdfs:label "Item - I32 13 K  When goods are Hong Kong originating goods"@en-AU ;
    dt:isPartOf C2004A04997:2 ;
    rdfs:comment "13 K  When goods are Hong Kong originating goods - Abrievated Graph Key: I32"@en-AU ;
    skos:definition "13 K  When goods are Hong Kong originating goods"@en-AU ;
    skos:narrower C2004A04997:2 ;
    skos:prefLabel "Item I32"@en-AU ;
    dcat:accessURL "https://www.legislation.gov.au/C2004A04997/2024-07-01/2024-07-01/text/1/epub/OEBPS/document_1/document_1.html#_Toc172806532"^^xsd:anyURI .

C2004A04997:320 a C2004A04997:Chapter ;
    rdfs:label "Chapter - C320 Chapter 74 Copper and articles thereof"@en-AU ;
    dt:isPartOf C2004A04997:318 ;
    rdfs:comment "Chapter 74 Copper and articles thereof - Abrievated Graph Key: C320"@en-AU ;
    skos:definition "Chapter 74 Copper and articles thereof"@en-AU ;
    skos:narrower C2004A04997:318 ;
    skos:prefLabel "Chapter C320"@en-AU ;
    dcat:accessURL "https://www.legislation.gov.au/C2004A04997/2024-07-01/2024-07-01/text/1/epub/OEBPS/document_5/document_5.html#_Toc171753162"^^xsd:anyURI .

C2004A04997:321 a C2004A04997:Item ;
    rdfs:label "Item - I321 Note"@en-AU ;
    dt:isPartOf C2004A04997:318 ;
    rdfs:comment "Note - Abrievated Graph Key: I321"@en-AU ;
    skos:definition "Note"@en-AU ;
    skos:narrower C2004A04997:318 ;
    skos:prefLabel "Item I321"@en-AU ;
    dcat:accessURL "https://www.legislation.gov.au/C2004A04997/2024-07-01/2024-07-01/text/1/epub/OEBPS/document_5/document_5.html#_Toc171753163"^^xsd:anyURI .

C2004A04997:322 a C2004A04997:Item ;
    rdfs:label "Item - I322 Subheading Note"@en-AU ;
    dt:isPartOf C2004A04997:318 ;
    rdfs:comment "Subheading Note - Abrievated Graph Key: I322"@en-AU ;
    skos:definition "Subheading Note"@en-AU ;
    skos:narrower C2004A04997:318 ;
    skos:prefLabel "Item I322"@en-AU ;
    dcat:accessURL "https://www.legislation.gov.au/C2004A04997/2024-07-01/2024-07-01/text/1/epub/OEBPS/document_5/document_5.html#_Toc171753164"^^xsd:anyURI .

C2004A04997:323 a C2004A04997:Chapter ;
    rdfs:label "Chapter - C323 Chapter 75 Nickel and articles thereof"@en-AU ;
    dt:isPartOf C2004A04997:318 ;
    rdfs:comment "Chapter 75 Nickel and articles thereof - Abrievated Graph Key: C323"@en-AU ;
    skos:definition "Chapter 75 Nickel and articles thereof"@en-AU ;
    skos:narrower C2004A04997:318 ;
    skos:prefLabel "Chapter C323"@en-AU ;
    dcat:accessURL "https://www.legislation.gov.au/C2004A04997/2024-07-01/2024-07-01/text/1/epub/OEBPS/document_5/document_5.html#_Toc171753165"^^xsd:anyURI .

C2004A04997:324 a C2004A04997:Item ;
    rdfs:label "Item - I324 Subheading Notes"@en-AU ;
    dt:isPartOf C2004A04997:318 ;
    rdfs:comment "Subheading Notes - Abrievated Graph Key: I324"@en-AU ;
    skos:definition "Subheading Notes"@en-AU ;
    skos:narrower C2004A04997:318 ;
    skos:prefLabel "Item I324"@en-AU ;
    dcat:accessURL "https://www.legislation.gov.au/C2004A04997/2024-07-01/2024-07-01/text/1/epub/OEBPS/document_5/document_5.html#_Toc171753166"^^xsd:anyURI .

C2004A04997:325 a C2004A04997:Chapter ;
    rdfs:label "Chapter - C325 Chapter 76 Aluminium and articles thereof"@en-AU ;
    dt:isPartOf C2004A04997:318 ;
    rdfs:comment "Chapter 76 Aluminium and articles thereof - Abrievated Graph Key: C325"@en-AU ;
    skos:definition "Chapter 76 Aluminium and articles thereof"@en-AU ;
    skos:narrower C2004A04997:318 ;
    skos:prefLabel "Chapter C325"@en-AU ;
    dcat:accessURL "https://www.legislation.gov.au/C2004A04997/2024-07-01/2024-07-01/text/1/epub/OEBPS/document_5/document_5.html#_Toc171753167"^^xsd:anyURI .

C2004A04997:326 a C2004A04997:Item ;
    rdfs:label "Item - I326 Subheading Notes"@en-AU ;
    dt:isPartOf C2004A04997:318 ;
    rdfs:comment "Subheading Notes - Abrievated Graph Key: I326"@en-AU ;
    skos:definition "Subheading Notes"@en-AU ;
    skos:narrower C2004A04997:318 ;
    skos:prefLabel "Item I326"@en-AU ;
    dcat:accessURL "https://www.legislation.gov.au/C2004A04997/2024-07-01/2024-07-01/text/1/epub/OEBPS/document_5/document_5.html#_Toc171753168"^^xsd:anyURI .

C2004A04997:327 a C2004A04997:Item ;
    rdfs:label "Item - I327 Additional Note"@en-AU ;
    dt:isPartOf C2004A04997:318 ;
    rdfs:comment "Additional Note - Abrievated Graph Key: I327"@en-AU ;
    skos:definition "Additional Note"@en-AU ;
    skos:narrower C2004A04997:318 ;
    skos:prefLabel "Item I327"@en-AU ;
    dcat:accessURL "https://www.legislation.gov.au/C2004A04997/2024-07-01/2024-07-01/text/1/epub/OEBPS/document_5/document_5.html#_Toc171753169"^^xsd:anyURI .

C2004A04997:328 a C2004A04997:Chapter ;
    rdfs:label "Chapter - C328 Chapter 78 Lead and articles thereof"@en-AU ;
    dt:isPartOf C2004A04997:318 ;
    rdfs:comment "Chapter 78 Lead and articles thereof - Abrievated Graph Key: C328"@en-AU ;
    skos:definition "Chapter 78 Lead and articles thereof"@en-AU ;
    skos:narrower C2004A04997:318 ;
    skos:prefLabel "Chapter C328"@en-AU ;
    dcat:accessURL "https://www.legislation.gov.au/C2004A04997/2024-07-01/2024-07-01/text/1/epub/OEBPS/document_5/document_5.html#_Toc171753170"^^xsd:anyURI .

C2004A04997:329 a C2004A04997:Item ;
    rdfs:label "Item - I329 Subheading Note"@en-AU ;
    dt:isPartOf C2004A04997:318 ;
    rdfs:comment "Subheading Note - Abrievated Graph Key: I329"@en-AU ;
    skos:definition "Subheading Note"@en-AU ;
    skos:narrower C2004A04997:318 ;
    skos:prefLabel "Item I329"@en-AU ;
    dcat:accessURL "https://www.legislation.gov.au/C2004A04997/2024-07-01/2024-07-01/text/1/epub/OEBPS/document_5/document_5.html#_Toc171753171"^^xsd:anyURI .

C2004A04997:33 a C2004A04997:Item ;
    rdfs:label "Item - I33 13 L  When goods are Regional Comprehensive Economic Partnership RCEP originating goods"@en-AU ;
    dt:isPartOf C2004A04997:2 ;
    rdfs:comment "13 L  When goods are Regional Comprehensive Economic Partnership RCEP originating goods - Abrievated Graph Key: I33"@en-AU ;
    skos:definition "13 L  When goods are Regional Comprehensive Economic Partnership RCEP originating goods"@en-AU ;
    skos:narrower C2004A04997:2 ;
    skos:prefLabel "Item I33"@en-AU ;
    dcat:accessURL "https://www.legislation.gov.au/C2004A04997/2024-07-01/2024-07-01/text/1/epub/OEBPS/document_1/document_1.html#_Toc172806533"^^xsd:anyURI .

C2004A04997:330 a C2004A04997:Chapter ;
    rdfs:label "Chapter - C330 Chapter 79 Zinc and articles thereof"@en-AU ;
    dt:isPartOf C2004A04997:318 ;
    rdfs:comment "Chapter 79 Zinc and articles thereof - Abrievated Graph Key: C330"@en-AU ;
    skos:definition "Chapter 79 Zinc and articles thereof"@en-AU ;
    skos:narrower C2004A04997:318 ;
    skos:prefLabel "Chapter C330"@en-AU ;
    dcat:accessURL "https://www.legislation.gov.au/C2004A04997/2024-07-01/2024-07-01/text/1/epub/OEBPS/document_5/document_5.html#_Toc171753172"^^xsd:anyURI .

C2004A04997:331 a C2004A04997:Item ;
    rdfs:label "Item - I331 Subheading Note"@en-AU ;
    dt:isPartOf C2004A04997:318 ;
    rdfs:comment "Subheading Note - Abrievated Graph Key: I331"@en-AU ;
    skos:definition "Subheading Note"@en-AU ;
    skos:narrower C2004A04997:318 ;
    skos:prefLabel "Item I331"@en-AU ;
    dcat:accessURL "https://www.legislation.gov.au/C2004A04997/2024-07-01/2024-07-01/text/1/epub/OEBPS/document_5/document_5.html#_Toc171753173"^^xsd:anyURI .

C2004A04997:332 a C2004A04997:Chapter ;
    rdfs:label "Chapter - C332 Chapter 80 Tin and articles thereof"@en-AU ;
    dt:isPartOf C2004A04997:318 ;
    rdfs:comment "Chapter 80 Tin and articles thereof - Abrievated Graph Key: C332"@en-AU ;
    skos:definition "Chapter 80 Tin and articles thereof"@en-AU ;
    skos:narrower C2004A04997:318 ;
    skos:prefLabel "Chapter C332"@en-AU ;
    dcat:accessURL "https://www.legislation.gov.au/C2004A04997/2024-07-01/2024-07-01/text/1/epub/OEBPS/document_5/document_5.html#_Toc171753174"^^xsd:anyURI .

C2004A04997:333 a C2004A04997:Item ;
    rdfs:label "Item - I333 Subheading Note"@en-AU ;
    dt:isPartOf C2004A04997:318 ;
    rdfs:comment "Subheading Note - Abrievated Graph Key: I333"@en-AU ;
    skos:definition "Subheading Note"@en-AU ;
    skos:narrower C2004A04997:318 ;
    skos:prefLabel "Item I333"@en-AU ;
    dcat:accessURL "https://www.legislation.gov.au/C2004A04997/2024-07-01/2024-07-01/text/1/epub/OEBPS/document_5/document_5.html#_Toc171753175"^^xsd:anyURI .

C2004A04997:334 a C2004A04997:Chapter ;
    rdfs:label "Chapter - C334 Chapter 81 Other base metals cermets articles thereof"@en-AU ;
    dt:isPartOf C2004A04997:318 ;
    rdfs:comment "Chapter 81 Other base metals cermets articles thereof - Abrievated Graph Key: C334"@en-AU ;
    skos:definition "Chapter 81 Other base metals cermets articles thereof"@en-AU ;
    skos:narrower C2004A04997:318 ;
    skos:prefLabel "Chapter C334"@en-AU ;
    dcat:accessURL "https://www.legislation.gov.au/C2004A04997/2024-07-01/2024-07-01/text/1/epub/OEBPS/document_5/document_5.html#_Toc171753176"^^xsd:anyURI .

C2004A04997:335 a C2004A04997:Chapter ;
    rdfs:label "Chapter - C335 Chapter 82 Tools implements cutlery spoons and forks of base metal parts thereof of base metal"@en-AU ;
    dt:isPartOf C2004A04997:318 ;
    rdfs:comment "Chapter 82 Tools implements cutlery spoons and forks of base metal parts thereof of base metal - Abrievated Graph Key: C335"@en-AU ;
    skos:definition "Chapter 82 Tools implements cutlery spoons and forks of base metal parts thereof of base metal"@en-AU ;
    skos:narrower C2004A04997:318 ;
    skos:prefLabel "Chapter C335"@en-AU ;
    dcat:accessURL "https://www.legislation.gov.au/C2004A04997/2024-07-01/2024-07-01/text/1/epub/OEBPS/document_5/document_5.html#_Toc171753177"^^xsd:anyURI .

C2004A04997:336 a C2004A04997:Item ;
    rdfs:label "Item - I336 Notes"@en-AU ;
    dt:isPartOf C2004A04997:318 ;
    rdfs:comment "Notes - Abrievated Graph Key: I336"@en-AU ;
    skos:definition "Notes"@en-AU ;
    skos:narrower C2004A04997:318 ;
    skos:prefLabel "Item I336"@en-AU ;
    dcat:accessURL "https://www.legislation.gov.au/C2004A04997/2024-07-01/2024-07-01/text/1/epub/OEBPS/document_5/document_5.html#_Toc171753178"^^xsd:anyURI .

C2004A04997:337 a C2004A04997:Chapter ;
    rdfs:label "Chapter - C337 Chapter 83 Miscellaneous articles of base metal"@en-AU ;
    dt:isPartOf C2004A04997:318 ;
    rdfs:comment "Chapter 83 Miscellaneous articles of base metal - Abrievated Graph Key: C337"@en-AU ;
    skos:definition "Chapter 83 Miscellaneous articles of base metal"@en-AU ;
    skos:narrower C2004A04997:318 ;
    skos:prefLabel "Chapter C337"@en-AU ;
    dcat:accessURL "https://www.legislation.gov.au/C2004A04997/2024-07-01/2024-07-01/text/1/epub/OEBPS/document_5/document_5.html#_Toc171753179"^^xsd:anyURI .

C2004A04997:338 a C2004A04997:Item ;
    rdfs:label "Item - I338 Notes"@en-AU ;
    dt:isPartOf C2004A04997:318 ;
    rdfs:comment "Notes - Abrievated Graph Key: I338"@en-AU ;
    skos:definition "Notes"@en-AU ;
    skos:narrower C2004A04997:318 ;
    skos:prefLabel "Item I338"@en-AU ;
    dcat:accessURL "https://www.legislation.gov.au/C2004A04997/2024-07-01/2024-07-01/text/1/epub/OEBPS/document_5/document_5.html#_Toc171753180"^^xsd:anyURI .

C2004A04997:339 a C2004A04997:Item ;
    rdfs:label "Item - I339 Additional Note"@en-AU ;
    dt:isPartOf C2004A04997:318 ;
    rdfs:comment "Additional Note - Abrievated Graph Key: I339"@en-AU ;
    skos:definition "Additional Note"@en-AU ;
    skos:narrower C2004A04997:318 ;
    skos:prefLabel "Item I339"@en-AU ;
    dcat:accessURL "https://www.legislation.gov.au/C2004A04997/2024-07-01/2024-07-01/text/1/epub/OEBPS/document_5/document_5.html#_Toc171753181"^^xsd:anyURI .

C2004A04997:34 a C2004A04997:Item ;
    rdfs:label "Item - I34 13 M  When goods are UK originating goods"@en-AU ;
    dt:isPartOf C2004A04997:2 ;
    rdfs:comment "13 M  When goods are UK originating goods - Abrievated Graph Key: I34"@en-AU ;
    skos:definition "13 M  When goods are UK originating goods"@en-AU ;
    skos:narrower C2004A04997:2 ;
    skos:prefLabel "Item I34"@en-AU ;
    dcat:accessURL "https://www.legislation.gov.au/C2004A04997/2024-07-01/2024-07-01/text/1/epub/OEBPS/document_1/document_1.html#_Toc172806534"^^xsd:anyURI .

C2004A04997:340 a C2004A04997:Section ;
    rdfs:label "Section - S340 Section XVIMachinery and mechanical appliances electrical equipment parts thereof sound recorders and reproducers television image and sound recorders and reproducers and parts and accessories of such articles"@en-AU ;
    dt:isPartOf C2004A04997:318 ;
    rdfs:comment "Section XVIMachinery and mechanical appliances electrical equipment parts thereof sound recorders and reproducers television image and sound recorders and reproducers and parts and accessories of such articles - Abrievated Graph Key: S340"@en-AU ;
    skos:definition "Section XVIMachinery and mechanical appliances electrical equipment parts thereof sound recorders and reproducers television image and sound recorders and reproducers and parts and accessories of such articles"@en-AU ;
    skos:narrower C2004A04997:318 ;
    skos:prefLabel "Section S340"@en-AU ;
    dcat:accessURL "https://www.legislation.gov.au/C2004A04997/2024-07-01/2024-07-01/text/1/epub/OEBPS/document_5/document_5.html#_Toc171753182"^^xsd:anyURI .

C2004A04997:341 a C2004A04997:Item ;
    rdfs:label "Item - I341 Notes"@en-AU ;
    dt:isPartOf C2004A04997:318 ;
    rdfs:comment "Notes - Abrievated Graph Key: I341"@en-AU ;
    skos:definition "Notes"@en-AU ;
    skos:narrower C2004A04997:318 ;
    skos:prefLabel "Item I341"@en-AU ;
    dcat:accessURL "https://www.legislation.gov.au/C2004A04997/2024-07-01/2024-07-01/text/1/epub/OEBPS/document_5/document_5.html#_Toc171753183"^^xsd:anyURI .

C2004A04997:342 a C2004A04997:Item ;
    rdfs:label "Item - I342 Additional Notes"@en-AU ;
    dt:isPartOf C2004A04997:318 ;
    rdfs:comment "Additional Notes - Abrievated Graph Key: I342"@en-AU ;
    skos:definition "Additional Notes"@en-AU ;
    skos:narrower C2004A04997:318 ;
    skos:prefLabel "Item I342"@en-AU ;
    dcat:accessURL "https://www.legislation.gov.au/C2004A04997/2024-07-01/2024-07-01/text/1/epub/OEBPS/document_5/document_5.html#_Toc171753184"^^xsd:anyURI .

C2004A04997:343 a C2004A04997:Chapter ;
    rdfs:label "Chapter - C343 Chapter 84 Nuclear reactors boilers machinery and mechanical appliances parts thereof"@en-AU ;
    dt:isPartOf C2004A04997:318 ;
    rdfs:comment "Chapter 84 Nuclear reactors boilers machinery and mechanical appliances parts thereof - Abrievated Graph Key: C343"@en-AU ;
    skos:definition "Chapter 84 Nuclear reactors boilers machinery and mechanical appliances parts thereof"@en-AU ;
    skos:narrower C2004A04997:318 ;
    skos:prefLabel "Chapter C343"@en-AU ;
    dcat:accessURL "https://www.legislation.gov.au/C2004A04997/2024-07-01/2024-07-01/text/1/epub/OEBPS/document_5/document_5.html#_Toc171753185"^^xsd:anyURI .

C2004A04997:344 a C2004A04997:Item ;
    rdfs:label "Item - I344 Notes"@en-AU ;
    dt:isPartOf C2004A04997:318 ;
    rdfs:comment "Notes - Abrievated Graph Key: I344"@en-AU ;
    skos:definition "Notes"@en-AU ;
    skos:narrower C2004A04997:318 ;
    skos:prefLabel "Item I344"@en-AU ;
    dcat:accessURL "https://www.legislation.gov.au/C2004A04997/2024-07-01/2024-07-01/text/1/epub/OEBPS/document_5/document_5.html#_Toc171753186"^^xsd:anyURI .

C2004A04997:345 a C2004A04997:Item ;
    rdfs:label "Item - I345 Subheading Notes"@en-AU ;
    dt:isPartOf C2004A04997:318 ;
    rdfs:comment "Subheading Notes - Abrievated Graph Key: I345"@en-AU ;
    skos:definition "Subheading Notes"@en-AU ;
    skos:narrower C2004A04997:318 ;
    skos:prefLabel "Item I345"@en-AU ;
    dcat:accessURL "https://www.legislation.gov.au/C2004A04997/2024-07-01/2024-07-01/text/1/epub/OEBPS/document_5/document_5.html#_Toc171753187"^^xsd:anyURI .

C2004A04997:346 a C2004A04997:Item ;
    rdfs:label "Item - I346 Additional Notes"@en-AU ;
    dt:isPartOf C2004A04997:318 ;
    rdfs:comment "Additional Notes - Abrievated Graph Key: I346"@en-AU ;
    skos:definition "Additional Notes"@en-AU ;
    skos:narrower C2004A04997:318 ;
    skos:prefLabel "Item I346"@en-AU ;
    dcat:accessURL "https://www.legislation.gov.au/C2004A04997/2024-07-01/2024-07-01/text/1/epub/OEBPS/document_5/document_5.html#_Toc171753188"^^xsd:anyURI .

C2004A04997:347 a C2004A04997:Chapter ;
    rdfs:label "Chapter - C347 Chapter 85 Electrical machinery and equipment and parts thereof sound recorders and reproducers television image and sound recorders and reproducers and parts and accessories of such articles"@en-AU ;
    dt:isPartOf C2004A04997:318 ;
    rdfs:comment "Chapter 85 Electrical machinery and equipment and parts thereof sound recorders and reproducers television image and sound recorders and reproducers and parts and accessories of such articles - Abrievated Graph Key: C347"@en-AU ;
    skos:definition "Chapter 85 Electrical machinery and equipment and parts thereof sound recorders and reproducers television image and sound recorders and reproducers and parts and accessories of such articles"@en-AU ;
    skos:narrower C2004A04997:318 ;
    skos:prefLabel "Chapter C347"@en-AU ;
    dcat:accessURL "https://www.legislation.gov.au/C2004A04997/2024-07-01/2024-07-01/text/1/epub/OEBPS/document_5/document_5.html#_Toc171753189"^^xsd:anyURI .

C2004A04997:348 a C2004A04997:Item ;
    rdfs:label "Item - I348 Notes"@en-AU ;
    dt:isPartOf C2004A04997:318 ;
    rdfs:comment "Notes - Abrievated Graph Key: I348"@en-AU ;
    skos:definition "Notes"@en-AU ;
    skos:narrower C2004A04997:318 ;
    skos:prefLabel "Item I348"@en-AU ;
    dcat:accessURL "https://www.legislation.gov.au/C2004A04997/2024-07-01/2024-07-01/text/1/epub/OEBPS/document_5/document_5.html#_Toc171753190"^^xsd:anyURI .

C2004A04997:349 a C2004A04997:Item ;
    rdfs:label "Item - I349 Subheading Notes"@en-AU ;
    dt:isPartOf C2004A04997:318 ;
    rdfs:comment "Subheading Notes - Abrievated Graph Key: I349"@en-AU ;
    skos:definition "Subheading Notes"@en-AU ;
    skos:narrower C2004A04997:318 ;
    skos:prefLabel "Item I349"@en-AU ;
    dcat:accessURL "https://www.legislation.gov.au/C2004A04997/2024-07-01/2024-07-01/text/1/epub/OEBPS/document_5/document_5.html#_Toc171753191"^^xsd:anyURI .

C2004A04997:35 a C2004A04997:Item ;
    rdfs:label "Item - I35 14  Application of rates of duty in relation to countries and places"@en-AU ;
    dt:isPartOf C2004A04997:2 ;
    rdfs:comment "14  Application of rates of duty in relation to countries and places - Abrievated Graph Key: I35"@en-AU ;
    skos:definition "14  Application of rates of duty in relation to countries and places"@en-AU ;
    skos:narrower C2004A04997:2 ;
    skos:prefLabel "Item I35"@en-AU ;
    dcat:accessURL "https://www.legislation.gov.au/C2004A04997/2024-07-01/2024-07-01/text/1/epub/OEBPS/document_1/document_1.html#_Toc172806535"^^xsd:anyURI .

C2004A04997:350 a C2004A04997:Item ;
    rdfs:label "Item - I350 Additional Notes"@en-AU ;
    dt:isPartOf C2004A04997:318 ;
    rdfs:comment "Additional Notes - Abrievated Graph Key: I350"@en-AU ;
    skos:definition "Additional Notes"@en-AU ;
    skos:narrower C2004A04997:318 ;
    skos:prefLabel "Item I350"@en-AU ;
    dcat:accessURL "https://www.legislation.gov.au/C2004A04997/2024-07-01/2024-07-01/text/1/epub/OEBPS/document_5/document_5.html#_Toc171753192"^^xsd:anyURI .

C2004A04997:351 a C2004A04997:Section ;
    rdfs:label "Section - S351 Section XVIIVehicles aircraft vessels and associated transport equipment"@en-AU ;
    dt:isPartOf C2004A04997:318 ;
    rdfs:comment "Section XVIIVehicles aircraft vessels and associated transport equipment - Abrievated Graph Key: S351"@en-AU ;
    skos:definition "Section XVIIVehicles aircraft vessels and associated transport equipment"@en-AU ;
    skos:narrower C2004A04997:318 ;
    skos:prefLabel "Section S351"@en-AU ;
    dcat:accessURL "https://www.legislation.gov.au/C2004A04997/2024-07-01/2024-07-01/text/1/epub/OEBPS/document_5/document_5.html#_Toc171753193"^^xsd:anyURI .

C2004A04997:352 a C2004A04997:Item ;
    rdfs:label "Item - I352 Notes"@en-AU ;
    dt:isPartOf C2004A04997:318 ;
    rdfs:comment "Notes - Abrievated Graph Key: I352"@en-AU ;
    skos:definition "Notes"@en-AU ;
    skos:narrower C2004A04997:318 ;
    skos:prefLabel "Item I352"@en-AU ;
    dcat:accessURL "https://www.legislation.gov.au/C2004A04997/2024-07-01/2024-07-01/text/1/epub/OEBPS/document_5/document_5.html#_Toc171753194"^^xsd:anyURI .

C2004A04997:353 a C2004A04997:Chapter ;
    rdfs:label "Chapter - C353 Chapter 86 Railway or tramway locomotives rolling stock and parts thereof railway or tramway track fixtures and fittings and parts thereof mechanical including electro mechanical traffic signalling equipment of all kinds"@en-AU ;
    dt:isPartOf C2004A04997:318 ;
    rdfs:comment "Chapter 86 Railway or tramway locomotives rolling stock and parts thereof railway or tramway track fixtures and fittings and parts thereof mechanical including electro mechanical traffic signalling equipment of all kinds - Abrievated Graph Key: C353"@en-AU ;
    skos:definition "Chapter 86 Railway or tramway locomotives rolling stock and parts thereof railway or tramway track fixtures and fittings and parts thereof mechanical including electro mechanical traffic signalling equipment of all kinds"@en-AU ;
    skos:narrower C2004A04997:318 ;
    skos:prefLabel "Chapter C353"@en-AU ;
    dcat:accessURL "https://www.legislation.gov.au/C2004A04997/2024-07-01/2024-07-01/text/1/epub/OEBPS/document_5/document_5.html#_Toc171753195"^^xsd:anyURI .

C2004A04997:354 a C2004A04997:Item ;
    rdfs:label "Item - I354 Notes"@en-AU ;
    dt:isPartOf C2004A04997:318 ;
    rdfs:comment "Notes - Abrievated Graph Key: I354"@en-AU ;
    skos:definition "Notes"@en-AU ;
    skos:narrower C2004A04997:318 ;
    skos:prefLabel "Item I354"@en-AU ;
    dcat:accessURL "https://www.legislation.gov.au/C2004A04997/2024-07-01/2024-07-01/text/1/epub/OEBPS/document_5/document_5.html#_Toc171753196"^^xsd:anyURI .

C2004A04997:355 a C2004A04997:Chapter ;
    rdfs:label "Chapter - C355 Chapter 87 Vehicles other than railway or tramway rolling stock and parts and accessories thereof"@en-AU ;
    dt:isPartOf C2004A04997:318 ;
    rdfs:comment "Chapter 87 Vehicles other than railway or tramway rolling stock and parts and accessories thereof - Abrievated Graph Key: C355"@en-AU ;
    skos:definition "Chapter 87 Vehicles other than railway or tramway rolling stock and parts and accessories thereof"@en-AU ;
    skos:narrower C2004A04997:318 ;
    skos:prefLabel "Chapter C355"@en-AU ;
    dcat:accessURL "https://www.legislation.gov.au/C2004A04997/2024-07-01/2024-07-01/text/1/epub/OEBPS/document_5/document_5.html#_Toc171753197"^^xsd:anyURI .

C2004A04997:356 a C2004A04997:Item ;
    rdfs:label "Item - I356 Notes"@en-AU ;
    dt:isPartOf C2004A04997:318 ;
    rdfs:comment "Notes - Abrievated Graph Key: I356"@en-AU ;
    skos:definition "Notes"@en-AU ;
    skos:narrower C2004A04997:318 ;
    skos:prefLabel "Item I356"@en-AU ;
    dcat:accessURL "https://www.legislation.gov.au/C2004A04997/2024-07-01/2024-07-01/text/1/epub/OEBPS/document_5/document_5.html#_Toc171753198"^^xsd:anyURI .

C2004A04997:357 a C2004A04997:Item ;
    rdfs:label "Item - I357 Subheading Note"@en-AU ;
    dt:isPartOf C2004A04997:318 ;
    rdfs:comment "Subheading Note - Abrievated Graph Key: I357"@en-AU ;
    skos:definition "Subheading Note"@en-AU ;
    skos:narrower C2004A04997:318 ;
    skos:prefLabel "Item I357"@en-AU ;
    dcat:accessURL "https://www.legislation.gov.au/C2004A04997/2024-07-01/2024-07-01/text/1/epub/OEBPS/document_5/document_5.html#_Toc171753199"^^xsd:anyURI .

C2004A04997:358 a C2004A04997:Item ;
    rdfs:label "Item - I358 Additional Notes"@en-AU ;
    dt:isPartOf C2004A04997:318 ;
    rdfs:comment "Additional Notes - Abrievated Graph Key: I358"@en-AU ;
    skos:definition "Additional Notes"@en-AU ;
    skos:narrower C2004A04997:318 ;
    skos:prefLabel "Item I358"@en-AU ;
    dcat:accessURL "https://www.legislation.gov.au/C2004A04997/2024-07-01/2024-07-01/text/1/epub/OEBPS/document_5/document_5.html#_Toc171753200"^^xsd:anyURI .

C2004A04997:359 a C2004A04997:Chapter ;
    rdfs:label "Chapter - C359 Chapter 88 Aircraft spacecraft and parts thereof"@en-AU ;
    dt:isPartOf C2004A04997:318 ;
    rdfs:comment "Chapter 88 Aircraft spacecraft and parts thereof - Abrievated Graph Key: C359"@en-AU ;
    skos:definition "Chapter 88 Aircraft spacecraft and parts thereof"@en-AU ;
    skos:narrower C2004A04997:318 ;
    skos:prefLabel "Chapter C359"@en-AU ;
    dcat:accessURL "https://www.legislation.gov.au/C2004A04997/2024-07-01/2024-07-01/text/1/epub/OEBPS/document_5/document_5.html#_Toc171753201"^^xsd:anyURI .

C2004A04997:360 a C2004A04997:Item ;
    rdfs:label "Item - I360 Note"@en-AU ;
    dt:isPartOf C2004A04997:318 ;
    rdfs:comment "Note - Abrievated Graph Key: I360"@en-AU ;
    skos:definition "Note"@en-AU ;
    skos:narrower C2004A04997:318 ;
    skos:prefLabel "Item I360"@en-AU ;
    dcat:accessURL "https://www.legislation.gov.au/C2004A04997/2024-07-01/2024-07-01/text/1/epub/OEBPS/document_5/document_5.html#_Toc171753202"^^xsd:anyURI .

C2004A04997:361 a C2004A04997:Item ;
    rdfs:label "Item - I361 Subheading Notes"@en-AU ;
    dt:isPartOf C2004A04997:318 ;
    rdfs:comment "Subheading Notes - Abrievated Graph Key: I361"@en-AU ;
    skos:definition "Subheading Notes"@en-AU ;
    skos:narrower C2004A04997:318 ;
    skos:prefLabel "Item I361"@en-AU ;
    dcat:accessURL "https://www.legislation.gov.au/C2004A04997/2024-07-01/2024-07-01/text/1/epub/OEBPS/document_5/document_5.html#_Toc171753203"^^xsd:anyURI .

C2004A04997:362 a C2004A04997:Chapter ;
    rdfs:label "Chapter - C362 Chapter 89 Ships boats and floating structures"@en-AU ;
    dt:isPartOf C2004A04997:318 ;
    rdfs:comment "Chapter 89 Ships boats and floating structures - Abrievated Graph Key: C362"@en-AU ;
    skos:definition "Chapter 89 Ships boats and floating structures"@en-AU ;
    skos:narrower C2004A04997:318 ;
    skos:prefLabel "Chapter C362"@en-AU ;
    dcat:accessURL "https://www.legislation.gov.au/C2004A04997/2024-07-01/2024-07-01/text/1/epub/OEBPS/document_5/document_5.html#_Toc171753204"^^xsd:anyURI .

C2004A04997:363 a C2004A04997:Item ;
    rdfs:label "Item - I363 Note"@en-AU ;
    dt:isPartOf C2004A04997:318 ;
    rdfs:comment "Note - Abrievated Graph Key: I363"@en-AU ;
    skos:definition "Note"@en-AU ;
    skos:narrower C2004A04997:318 ;
    skos:prefLabel "Item I363"@en-AU ;
    dcat:accessURL "https://www.legislation.gov.au/C2004A04997/2024-07-01/2024-07-01/text/1/epub/OEBPS/document_5/document_5.html#_Toc171753205"^^xsd:anyURI .

C2004A04997:364 a C2004A04997:Section ;
    rdfs:label "Section - S364 Section XVIIIOptical photographic cinematographic measuring checking precision medical or surgical instruments and apparatus clocks and watches musical instruments parts and accessories thereof"@en-AU ;
    dt:isPartOf C2004A04997:318 ;
    rdfs:comment "Section XVIIIOptical photographic cinematographic measuring checking precision medical or surgical instruments and apparatus clocks and watches musical instruments parts and accessories thereof - Abrievated Graph Key: S364"@en-AU ;
    skos:definition "Section XVIIIOptical photographic cinematographic measuring checking precision medical or surgical instruments and apparatus clocks and watches musical instruments parts and accessories thereof"@en-AU ;
    skos:narrower C2004A04997:318 ;
    skos:prefLabel "Section S364"@en-AU ;
    dcat:accessURL "https://www.legislation.gov.au/C2004A04997/2024-07-01/2024-07-01/text/1/epub/OEBPS/document_5/document_5.html#_Toc171753206"^^xsd:anyURI .

C2004A04997:365 a C2004A04997:Chapter ;
    rdfs:label "Chapter - C365 Chapter 90 Optical photographic cinematographic measuring checking precision medical or surgical instruments and apparatus parts and accessories thereof"@en-AU ;
    dt:isPartOf C2004A04997:318 ;
    rdfs:comment "Chapter 90 Optical photographic cinematographic measuring checking precision medical or surgical instruments and apparatus parts and accessories thereof - Abrievated Graph Key: C365"@en-AU ;
    skos:definition "Chapter 90 Optical photographic cinematographic measuring checking precision medical or surgical instruments and apparatus parts and accessories thereof"@en-AU ;
    skos:narrower C2004A04997:318 ;
    skos:prefLabel "Chapter C365"@en-AU ;
    dcat:accessURL "https://www.legislation.gov.au/C2004A04997/2024-07-01/2024-07-01/text/1/epub/OEBPS/document_5/document_5.html#_Toc171753207"^^xsd:anyURI .

C2004A04997:366 a C2004A04997:Item ;
    rdfs:label "Item - I366 Notes"@en-AU ;
    dt:isPartOf C2004A04997:318 ;
    rdfs:comment "Notes - Abrievated Graph Key: I366"@en-AU ;
    skos:definition "Notes"@en-AU ;
    skos:narrower C2004A04997:318 ;
    skos:prefLabel "Item I366"@en-AU ;
    dcat:accessURL "https://www.legislation.gov.au/C2004A04997/2024-07-01/2024-07-01/text/1/epub/OEBPS/document_5/document_5.html#_Toc171753208"^^xsd:anyURI .

C2004A04997:367 a C2004A04997:Item ;
    rdfs:label "Item - I367 Additional Notes"@en-AU ;
    dt:isPartOf C2004A04997:318 ;
    rdfs:comment "Additional Notes - Abrievated Graph Key: I367"@en-AU ;
    skos:definition "Additional Notes"@en-AU ;
    skos:narrower C2004A04997:318 ;
    skos:prefLabel "Item I367"@en-AU ;
    dcat:accessURL "https://www.legislation.gov.au/C2004A04997/2024-07-01/2024-07-01/text/1/epub/OEBPS/document_5/document_5.html#_Toc171753209"^^xsd:anyURI .

C2004A04997:368 a C2004A04997:Chapter ;
    rdfs:label "Chapter - C368 Chapter 91 Clocks and watches and parts thereof"@en-AU ;
    dt:isPartOf C2004A04997:318 ;
    rdfs:comment "Chapter 91 Clocks and watches and parts thereof - Abrievated Graph Key: C368"@en-AU ;
    skos:definition "Chapter 91 Clocks and watches and parts thereof"@en-AU ;
    skos:narrower C2004A04997:318 ;
    skos:prefLabel "Chapter C368"@en-AU ;
    dcat:accessURL "https://www.legislation.gov.au/C2004A04997/2024-07-01/2024-07-01/text/1/epub/OEBPS/document_5/document_5.html#_Toc171753210"^^xsd:anyURI .

C2004A04997:369 a C2004A04997:Item ;
    rdfs:label "Item - I369 Notes"@en-AU ;
    dt:isPartOf C2004A04997:318 ;
    rdfs:comment "Notes - Abrievated Graph Key: I369"@en-AU ;
    skos:definition "Notes"@en-AU ;
    skos:narrower C2004A04997:318 ;
    skos:prefLabel "Item I369"@en-AU ;
    dcat:accessURL "https://www.legislation.gov.au/C2004A04997/2024-07-01/2024-07-01/text/1/epub/OEBPS/document_5/document_5.html#_Toc171753211"^^xsd:anyURI .

C2004A04997:37 a C2004A04997:Item ;
    rdfs:label "Item - I37 15  Imposition of duties"@en-AU ;
    dt:isPartOf C2004A04997:36 ;
    rdfs:comment "15  Imposition of duties - Abrievated Graph Key: I37"@en-AU ;
    skos:definition "15  Imposition of duties"@en-AU ;
    skos:narrower C2004A04997:36 ;
    skos:prefLabel "Item I37"@en-AU ;
    dcat:accessURL "https://www.legislation.gov.au/C2004A04997/2024-07-01/2024-07-01/text/1/epub/OEBPS/document_1/document_1.html#_Toc172806537"^^xsd:anyURI .

C2004A04997:370 a C2004A04997:Chapter ;
    rdfs:label "Chapter - C370 Chapter 92 Musical instruments parts and accessories of such articles"@en-AU ;
    dt:isPartOf C2004A04997:318 ;
    rdfs:comment "Chapter 92 Musical instruments parts and accessories of such articles - Abrievated Graph Key: C370"@en-AU ;
    skos:definition "Chapter 92 Musical instruments parts and accessories of such articles"@en-AU ;
    skos:narrower C2004A04997:318 ;
    skos:prefLabel "Chapter C370"@en-AU ;
    dcat:accessURL "https://www.legislation.gov.au/C2004A04997/2024-07-01/2024-07-01/text/1/epub/OEBPS/document_5/document_5.html#_Toc171753212"^^xsd:anyURI .

C2004A04997:371 a C2004A04997:Item ;
    rdfs:label "Item - I371 Notes"@en-AU ;
    dt:isPartOf C2004A04997:318 ;
    rdfs:comment "Notes - Abrievated Graph Key: I371"@en-AU ;
    skos:definition "Notes"@en-AU ;
    skos:narrower C2004A04997:318 ;
    skos:prefLabel "Item I371"@en-AU ;
    dcat:accessURL "https://www.legislation.gov.au/C2004A04997/2024-07-01/2024-07-01/text/1/epub/OEBPS/document_5/document_5.html#_Toc171753213"^^xsd:anyURI .

C2004A04997:372 a C2004A04997:Section ;
    rdfs:label "Section - S372 Section XIXArms and ammunition parts and accessories thereof"@en-AU ;
    dt:isPartOf C2004A04997:318 ;
    rdfs:comment "Section XIXArms and ammunition parts and accessories thereof - Abrievated Graph Key: S372"@en-AU ;
    skos:definition "Section XIXArms and ammunition parts and accessories thereof"@en-AU ;
    skos:narrower C2004A04997:318 ;
    skos:prefLabel "Section S372"@en-AU ;
    dcat:accessURL "https://www.legislation.gov.au/C2004A04997/2024-07-01/2024-07-01/text/1/epub/OEBPS/document_5/document_5.html#_Toc171753214"^^xsd:anyURI .

C2004A04997:373 a C2004A04997:Chapter ;
    rdfs:label "Chapter - C373 Chapter 93 Arms and ammunition parts and accessories thereof"@en-AU ;
    dt:isPartOf C2004A04997:318 ;
    rdfs:comment "Chapter 93 Arms and ammunition parts and accessories thereof - Abrievated Graph Key: C373"@en-AU ;
    skos:definition "Chapter 93 Arms and ammunition parts and accessories thereof"@en-AU ;
    skos:narrower C2004A04997:318 ;
    skos:prefLabel "Chapter C373"@en-AU ;
    dcat:accessURL "https://www.legislation.gov.au/C2004A04997/2024-07-01/2024-07-01/text/1/epub/OEBPS/document_5/document_5.html#_Toc171753215"^^xsd:anyURI .

C2004A04997:374 a C2004A04997:Item ;
    rdfs:label "Item - I374 Notes"@en-AU ;
    dt:isPartOf C2004A04997:318 ;
    rdfs:comment "Notes - Abrievated Graph Key: I374"@en-AU ;
    skos:definition "Notes"@en-AU ;
    skos:narrower C2004A04997:318 ;
    skos:prefLabel "Item I374"@en-AU ;
    dcat:accessURL "https://www.legislation.gov.au/C2004A04997/2024-07-01/2024-07-01/text/1/epub/OEBPS/document_5/document_5.html#_Toc171753216"^^xsd:anyURI .

C2004A04997:375 a C2004A04997:Section ;
    rdfs:label "Section - S375 Section XXMiscellaneous manufactured articles"@en-AU ;
    dt:isPartOf C2004A04997:318 ;
    rdfs:comment "Section XXMiscellaneous manufactured articles - Abrievated Graph Key: S375"@en-AU ;
    skos:definition "Section XXMiscellaneous manufactured articles"@en-AU ;
    skos:narrower C2004A04997:318 ;
    skos:prefLabel "Section S375"@en-AU ;
    dcat:accessURL "https://www.legislation.gov.au/C2004A04997/2024-07-01/2024-07-01/text/1/epub/OEBPS/document_5/document_5.html#_Toc171753217"^^xsd:anyURI .

C2004A04997:376 a C2004A04997:Chapter ;
    rdfs:label "Chapter - C376 Chapter 94 Furniture bedding mattresses mattress supports cushions and similar stuffed furnishings luminaires and lighting fittings not elsewhere specified or included illuminated signs illuminated name plates and the like prefabricated buildings"@en-AU ;
    dt:isPartOf C2004A04997:318 ;
    rdfs:comment "Chapter 94 Furniture bedding mattresses mattress supports cushions and similar stuffed furnishings luminaires and lighting fittings not elsewhere specified or included illuminated signs illuminated name plates and the like prefabricated buildings - Abrievated Graph Key: C376"@en-AU ;
    skos:definition "Chapter 94 Furniture bedding mattresses mattress supports cushions and similar stuffed furnishings luminaires and lighting fittings not elsewhere specified or included illuminated signs illuminated name plates and the like prefabricated buildings"@en-AU ;
    skos:narrower C2004A04997:318 ;
    skos:prefLabel "Chapter C376"@en-AU ;
    dcat:accessURL "https://www.legislation.gov.au/C2004A04997/2024-07-01/2024-07-01/text/1/epub/OEBPS/document_5/document_5.html#_Toc171753218"^^xsd:anyURI .

C2004A04997:377 a C2004A04997:Item ;
    rdfs:label "Item - I377 Notes"@en-AU ;
    dt:isPartOf C2004A04997:318 ;
    rdfs:comment "Notes - Abrievated Graph Key: I377"@en-AU ;
    skos:definition "Notes"@en-AU ;
    skos:narrower C2004A04997:318 ;
    skos:prefLabel "Item I377"@en-AU ;
    dcat:accessURL "https://www.legislation.gov.au/C2004A04997/2024-07-01/2024-07-01/text/1/epub/OEBPS/document_5/document_5.html#_Toc171753219"^^xsd:anyURI .

C2004A04997:378 a C2004A04997:Item ;
    rdfs:label "Item - I378 Additional Note"@en-AU ;
    dt:isPartOf C2004A04997:318 ;
    rdfs:comment "Additional Note - Abrievated Graph Key: I378"@en-AU ;
    skos:definition "Additional Note"@en-AU ;
    skos:narrower C2004A04997:318 ;
    skos:prefLabel "Item I378"@en-AU ;
    dcat:accessURL "https://www.legislation.gov.au/C2004A04997/2024-07-01/2024-07-01/text/1/epub/OEBPS/document_5/document_5.html#_Toc171753220"^^xsd:anyURI .

C2004A04997:379 a C2004A04997:Chapter ;
    rdfs:label "Chapter - C379 Chapter 95 Toys games and sports requisites parts and accessories thereof"@en-AU ;
    dt:isPartOf C2004A04997:318 ;
    rdfs:comment "Chapter 95 Toys games and sports requisites parts and accessories thereof - Abrievated Graph Key: C379"@en-AU ;
    skos:definition "Chapter 95 Toys games and sports requisites parts and accessories thereof"@en-AU ;
    skos:narrower C2004A04997:318 ;
    skos:prefLabel "Chapter C379"@en-AU ;
    dcat:accessURL "https://www.legislation.gov.au/C2004A04997/2024-07-01/2024-07-01/text/1/epub/OEBPS/document_5/document_5.html#_Toc171753221"^^xsd:anyURI .

C2004A04997:38 a C2004A04997:Item ;
    rdfs:label "Item - I38 16  Calculation of duty"@en-AU ;
    dt:isPartOf C2004A04997:36 ;
    rdfs:comment "16  Calculation of duty - Abrievated Graph Key: I38"@en-AU ;
    skos:definition "16  Calculation of duty"@en-AU ;
    skos:narrower C2004A04997:36 ;
    skos:prefLabel "Item I38"@en-AU ;
    dcat:accessURL "https://www.legislation.gov.au/C2004A04997/2024-07-01/2024-07-01/text/1/epub/OEBPS/document_1/document_1.html#_Toc172806538"^^xsd:anyURI .

C2004A04997:380 a C2004A04997:Item ;
    rdfs:label "Item - I380 Notes"@en-AU ;
    dt:isPartOf C2004A04997:318 ;
    rdfs:comment "Notes - Abrievated Graph Key: I380"@en-AU ;
    skos:definition "Notes"@en-AU ;
    skos:narrower C2004A04997:318 ;
    skos:prefLabel "Item I380"@en-AU ;
    dcat:accessURL "https://www.legislation.gov.au/C2004A04997/2024-07-01/2024-07-01/text/1/epub/OEBPS/document_5/document_5.html#_Toc171753222"^^xsd:anyURI .

C2004A04997:381 a C2004A04997:Item ;
    rdfs:label "Item - I381 Subheading Note"@en-AU ;
    dt:isPartOf C2004A04997:318 ;
    rdfs:comment "Subheading Note - Abrievated Graph Key: I381"@en-AU ;
    skos:definition "Subheading Note"@en-AU ;
    skos:narrower C2004A04997:318 ;
    skos:prefLabel "Item I381"@en-AU ;
    dcat:accessURL "https://www.legislation.gov.au/C2004A04997/2024-07-01/2024-07-01/text/1/epub/OEBPS/document_5/document_5.html#_Toc171753223"^^xsd:anyURI .

C2004A04997:382 a C2004A04997:Chapter ;
    rdfs:label "Chapter - C382 Chapter 96 Miscellaneous manufactured articles"@en-AU ;
    dt:isPartOf C2004A04997:318 ;
    rdfs:comment "Chapter 96 Miscellaneous manufactured articles - Abrievated Graph Key: C382"@en-AU ;
    skos:definition "Chapter 96 Miscellaneous manufactured articles"@en-AU ;
    skos:narrower C2004A04997:318 ;
    skos:prefLabel "Chapter C382"@en-AU ;
    dcat:accessURL "https://www.legislation.gov.au/C2004A04997/2024-07-01/2024-07-01/text/1/epub/OEBPS/document_5/document_5.html#_Toc171753224"^^xsd:anyURI .

C2004A04997:383 a C2004A04997:Item ;
    rdfs:label "Item - I383 Notes"@en-AU ;
    dt:isPartOf C2004A04997:318 ;
    rdfs:comment "Notes - Abrievated Graph Key: I383"@en-AU ;
    skos:definition "Notes"@en-AU ;
    skos:narrower C2004A04997:318 ;
    skos:prefLabel "Item I383"@en-AU ;
    dcat:accessURL "https://www.legislation.gov.au/C2004A04997/2024-07-01/2024-07-01/text/1/epub/OEBPS/document_5/document_5.html#_Toc171753225"^^xsd:anyURI .

C2004A04997:384 a C2004A04997:Section ;
    rdfs:label "Section - S384 Section XXIWorks of art collectors pieces and antiques"@en-AU ;
    dt:isPartOf C2004A04997:318 ;
    rdfs:comment "Section XXIWorks of art collectors pieces and antiques - Abrievated Graph Key: S384"@en-AU ;
    skos:definition "Section XXIWorks of art collectors pieces and antiques"@en-AU ;
    skos:narrower C2004A04997:318 ;
    skos:prefLabel "Section S384"@en-AU ;
    dcat:accessURL "https://www.legislation.gov.au/C2004A04997/2024-07-01/2024-07-01/text/1/epub/OEBPS/document_5/document_5.html#_Toc171753226"^^xsd:anyURI .

C2004A04997:385 a C2004A04997:Chapter ;
    rdfs:label "Chapter - C385 Chapter 97 Works of art collectors pieces and antiques"@en-AU ;
    dt:isPartOf C2004A04997:318 ;
    rdfs:comment "Chapter 97 Works of art collectors pieces and antiques - Abrievated Graph Key: C385"@en-AU ;
    skos:definition "Chapter 97 Works of art collectors pieces and antiques"@en-AU ;
    skos:narrower C2004A04997:318 ;
    skos:prefLabel "Chapter C385"@en-AU ;
    dcat:accessURL "https://www.legislation.gov.au/C2004A04997/2024-07-01/2024-07-01/text/1/epub/OEBPS/document_5/document_5.html#_Toc171753227"^^xsd:anyURI .

C2004A04997:386 a C2004A04997:Item ;
    rdfs:label "Item - I386 Notes"@en-AU ;
    dt:isPartOf C2004A04997:318 ;
    rdfs:comment "Notes - Abrievated Graph Key: I386"@en-AU ;
    skos:definition "Notes"@en-AU ;
    skos:narrower C2004A04997:318 ;
    skos:prefLabel "Item I386"@en-AU ;
    dcat:accessURL "https://www.legislation.gov.au/C2004A04997/2024-07-01/2024-07-01/text/1/epub/OEBPS/document_5/document_5.html#_Toc171753228"^^xsd:anyURI .

C2004A04997:387 a C2004A04997:Item ;
    rdfs:label "Item - I387 Additional Notes"@en-AU ;
    dt:isPartOf C2004A04997:318 ;
    rdfs:comment "Additional Notes - Abrievated Graph Key: I387"@en-AU ;
    skos:definition "Additional Notes"@en-AU ;
    skos:narrower C2004A04997:318 ;
    skos:prefLabel "Item I387"@en-AU ;
    dcat:accessURL "https://www.legislation.gov.au/C2004A04997/2024-07-01/2024-07-01/text/1/epub/OEBPS/document_5/document_5.html#_Toc171753229"^^xsd:anyURI .

C2004A04997:389 a C2004A04997:Schedule ;
    rdfs:label "Schedule - S389 Schedule 4 Concessional rates of duty"@en-AU ;
    dt:isPartOf C2004A04997:388 ;
    rdfs:comment "Schedule 4 Concessional rates of duty - Abrievated Graph Key: S389"@en-AU ;
    skos:definition "Schedule 4 Concessional rates of duty"@en-AU ;
    skos:narrower C2004A04997:388 ;
    skos:prefLabel "Schedule S389"@en-AU ;
    dcat:accessURL "https://www.legislation.gov.au/C2004A04997/2024-07-01/2024-07-01/text/1/epub/OEBPS/document_6/document_6.html#_Toc171754999"^^xsd:anyURI .

C2004A04997:39 a C2004A04997:Item ;
    rdfs:label "Item - I39 16 A  Suspension of preferential tariff for UK originating goodssafeguard goods"@en-AU ;
    dt:isPartOf C2004A04997:36 ;
    rdfs:comment "16 A  Suspension of preferential tariff for UK originating goodssafeguard goods - Abrievated Graph Key: I39"@en-AU ;
    skos:definition "16 A  Suspension of preferential tariff for UK originating goodssafeguard goods"@en-AU ;
    skos:narrower C2004A04997:36 ;
    skos:prefLabel "Item I39"@en-AU ;
    dcat:accessURL "https://www.legislation.gov.au/C2004A04997/2024-07-01/2024-07-01/text/1/epub/OEBPS/document_1/document_1.html#_Toc172806539"^^xsd:anyURI .

C2004A04997:390 a C2004A04997:Schedule ;
    rdfs:label "Schedule - S390 Schedule 4 ASingaporean originating goods"@en-AU ;
    dt:isPartOf C2004A04997:388 ;
    rdfs:comment "Schedule 4 ASingaporean originating goods - Abrievated Graph Key: S390"@en-AU ;
    skos:definition "Schedule 4 ASingaporean originating goods"@en-AU ;
    skos:narrower C2004A04997:388 ;
    skos:prefLabel "Schedule S390"@en-AU ;
    dcat:accessURL "https://www.legislation.gov.au/C2004A04997/2024-07-01/2024-07-01/text/1/epub/OEBPS/document_6/document_6.html#_Toc171755000"^^xsd:anyURI .

C2004A04997:391 a C2004A04997:Schedule ;
    rdfs:label "Schedule - S391 Schedule 5 US originating goods"@en-AU ;
    dt:isPartOf C2004A04997:388 ;
    rdfs:comment "Schedule 5 US originating goods - Abrievated Graph Key: S391"@en-AU ;
    skos:definition "Schedule 5 US originating goods"@en-AU ;
    skos:narrower C2004A04997:388 ;
    skos:prefLabel "Schedule S391"@en-AU ;
    dcat:accessURL "https://www.legislation.gov.au/C2004A04997/2024-07-01/2024-07-01/text/1/epub/OEBPS/document_6/document_6.html#_Toc171755001"^^xsd:anyURI .

C2004A04997:392 a C2004A04997:Schedule ;
    rdfs:label "Schedule - S392 Schedule 6 Thai originating goods"@en-AU ;
    dt:isPartOf C2004A04997:388 ;
    rdfs:comment "Schedule 6 Thai originating goods - Abrievated Graph Key: S392"@en-AU ;
    skos:definition "Schedule 6 Thai originating goods"@en-AU ;
    skos:narrower C2004A04997:388 ;
    skos:prefLabel "Schedule S392"@en-AU ;
    dcat:accessURL "https://www.legislation.gov.au/C2004A04997/2024-07-01/2024-07-01/text/1/epub/OEBPS/document_6/document_6.html#_Toc171755002"^^xsd:anyURI .

C2004A04997:393 a C2004A04997:Schedule ;
    rdfs:label "Schedule - S393 Schedule 6 APeruvian originating goods"@en-AU ;
    dt:isPartOf C2004A04997:388 ;
    rdfs:comment "Schedule 6 APeruvian originating goods - Abrievated Graph Key: S393"@en-AU ;
    skos:definition "Schedule 6 APeruvian originating goods"@en-AU ;
    skos:narrower C2004A04997:388 ;
    skos:prefLabel "Schedule S393"@en-AU ;
    dcat:accessURL "https://www.legislation.gov.au/C2004A04997/2024-07-01/2024-07-01/text/1/epub/OEBPS/document_6/document_6.html#_Toc171755003"^^xsd:anyURI .

C2004A04997:394 a C2004A04997:Schedule ;
    rdfs:label "Schedule - S394 Schedule 7 Chilean originating goods"@en-AU ;
    dt:isPartOf C2004A04997:388 ;
    rdfs:comment "Schedule 7 Chilean originating goods - Abrievated Graph Key: S394"@en-AU ;
    skos:definition "Schedule 7 Chilean originating goods"@en-AU ;
    skos:narrower C2004A04997:388 ;
    skos:prefLabel "Schedule S394"@en-AU ;
    dcat:accessURL "https://www.legislation.gov.au/C2004A04997/2024-07-01/2024-07-01/text/1/epub/OEBPS/document_6/document_6.html#_Toc171755004"^^xsd:anyURI .

C2004A04997:395 a C2004A04997:Schedule ;
    rdfs:label "Schedule - S395 Schedule 8 ASEAN Australia New Zealand AANZ originating goods"@en-AU ;
    dt:isPartOf C2004A04997:388 ;
    rdfs:comment "Schedule 8 ASEAN Australia New Zealand AANZ originating goods - Abrievated Graph Key: S395"@en-AU ;
    skos:definition "Schedule 8 ASEAN Australia New Zealand AANZ originating goods"@en-AU ;
    skos:narrower C2004A04997:388 ;
    skos:prefLabel "Schedule S395"@en-AU ;
    dcat:accessURL "https://www.legislation.gov.au/C2004A04997/2024-07-01/2024-07-01/text/1/epub/OEBPS/document_6/document_6.html#_Toc171755005"^^xsd:anyURI .

C2004A04997:396 a C2004A04997:Schedule ;
    rdfs:label "Schedule - S396 Schedule 8 APacific Islands originating goods"@en-AU ;
    dt:isPartOf C2004A04997:388 ;
    rdfs:comment "Schedule 8 APacific Islands originating goods - Abrievated Graph Key: S396"@en-AU ;
    skos:definition "Schedule 8 APacific Islands originating goods"@en-AU ;
    skos:narrower C2004A04997:388 ;
    skos:prefLabel "Schedule S396"@en-AU ;
    dcat:accessURL "https://www.legislation.gov.au/C2004A04997/2024-07-01/2024-07-01/text/1/epub/OEBPS/document_6/document_6.html#_Toc171755006"^^xsd:anyURI .

C2004A04997:397 a C2004A04997:Schedule ;
    rdfs:label "Schedule - S397 Schedule 8 BTrans Pacific Partnership originating goods"@en-AU ;
    dt:isPartOf C2004A04997:388 ;
    rdfs:comment "Schedule 8 BTrans Pacific Partnership originating goods - Abrievated Graph Key: S397"@en-AU ;
    skos:definition "Schedule 8 BTrans Pacific Partnership originating goods"@en-AU ;
    skos:narrower C2004A04997:388 ;
    skos:prefLabel "Schedule S397"@en-AU ;
    dcat:accessURL "https://www.legislation.gov.au/C2004A04997/2024-07-01/2024-07-01/text/1/epub/OEBPS/document_6/document_6.html#_Toc171755007"^^xsd:anyURI .

C2004A04997:398 a C2004A04997:Schedule ;
    rdfs:label "Schedule - S398 Schedule 9 Malaysian originating goods"@en-AU ;
    dt:isPartOf C2004A04997:388 ;
    rdfs:comment "Schedule 9 Malaysian originating goods - Abrievated Graph Key: S398"@en-AU ;
    skos:definition "Schedule 9 Malaysian originating goods"@en-AU ;
    skos:narrower C2004A04997:388 ;
    skos:prefLabel "Schedule S398"@en-AU ;
    dcat:accessURL "https://www.legislation.gov.au/C2004A04997/2024-07-01/2024-07-01/text/1/epub/OEBPS/document_6/document_6.html#_Toc171755008"^^xsd:anyURI .

C2004A04997:399 a C2004A04997:Schedule ;
    rdfs:label "Schedule - S399 Schedule 9 AIndonesian originating goods"@en-AU ;
    dt:isPartOf C2004A04997:388 ;
    rdfs:comment "Schedule 9 AIndonesian originating goods - Abrievated Graph Key: S399"@en-AU ;
    skos:definition "Schedule 9 AIndonesian originating goods"@en-AU ;
    skos:narrower C2004A04997:388 ;
    skos:prefLabel "Schedule S399"@en-AU ;
    dcat:accessURL "https://www.legislation.gov.au/C2004A04997/2024-07-01/2024-07-01/text/1/epub/OEBPS/document_6/document_6.html#_Toc171755009"^^xsd:anyURI .

C2004A04997:4 a C2004A04997:Item ;
    rdfs:label "Item - I4 2  Commencement"@en-AU ;
    dt:isPartOf C2004A04997:2 ;
    rdfs:comment "2  Commencement - Abrievated Graph Key: I4"@en-AU ;
    skos:definition "2  Commencement"@en-AU ;
    skos:narrower C2004A04997:2 ;
    skos:prefLabel "Item I4"@en-AU ;
    dcat:accessURL "https://www.legislation.gov.au/C2004A04997/2024-07-01/2024-07-01/text/1/epub/OEBPS/document_1/document_1.html#_Toc172806504"^^xsd:anyURI .

C2004A04997:40 a C2004A04997:Item ;
    rdfs:label "Item - I40 17  Rates for goods with constituents etc"@en-AU ;
    dt:isPartOf C2004A04997:36 ;
    rdfs:comment "17  Rates for goods with constituents etc - Abrievated Graph Key: I40"@en-AU ;
    skos:definition "17  Rates for goods with constituents etc"@en-AU ;
    skos:narrower C2004A04997:36 ;
    skos:prefLabel "Item I40"@en-AU ;
    dcat:accessURL "https://www.legislation.gov.au/C2004A04997/2024-07-01/2024-07-01/text/1/epub/OEBPS/document_1/document_1.html#_Toc172806540"^^xsd:anyURI .

C2004A04997:400 a C2004A04997:Schedule ;
    rdfs:label "Schedule - S400 Schedule 10 Korean originating goods"@en-AU ;
    dt:isPartOf C2004A04997:388 ;
    rdfs:comment "Schedule 10 Korean originating goods - Abrievated Graph Key: S400"@en-AU ;
    skos:definition "Schedule 10 Korean originating goods"@en-AU ;
    skos:narrower C2004A04997:388 ;
    skos:prefLabel "Schedule S400"@en-AU ;
    dcat:accessURL "https://www.legislation.gov.au/C2004A04997/2024-07-01/2024-07-01/text/1/epub/OEBPS/document_6/document_6.html#_Toc171755010"^^xsd:anyURI .

C2004A04997:401 a C2004A04997:Schedule ;
    rdfs:label "Schedule - S401 Schedule 10 AIndian originating goods"@en-AU ;
    dt:isPartOf C2004A04997:388 ;
    rdfs:comment "Schedule 10 AIndian originating goods - Abrievated Graph Key: S401"@en-AU ;
    skos:definition "Schedule 10 AIndian originating goods"@en-AU ;
    skos:narrower C2004A04997:388 ;
    skos:prefLabel "Schedule S401"@en-AU ;
    dcat:accessURL "https://www.legislation.gov.au/C2004A04997/2024-07-01/2024-07-01/text/1/epub/OEBPS/document_6/document_6.html#_Toc171755011"^^xsd:anyURI .

C2004A04997:402 a C2004A04997:Schedule ;
    rdfs:label "Schedule - S402 Schedule 11 Japanese originating goods"@en-AU ;
    dt:isPartOf C2004A04997:388 ;
    rdfs:comment "Schedule 11 Japanese originating goods - Abrievated Graph Key: S402"@en-AU ;
    skos:definition "Schedule 11 Japanese originating goods"@en-AU ;
    skos:narrower C2004A04997:388 ;
    skos:prefLabel "Schedule S402"@en-AU ;
    dcat:accessURL "https://www.legislation.gov.au/C2004A04997/2024-07-01/2024-07-01/text/1/epub/OEBPS/document_6/document_6.html#_Toc171755012"^^xsd:anyURI .

C2004A04997:403 a C2004A04997:Schedule ;
    rdfs:label "Schedule - S403 Schedule 12 Chinese originating goods"@en-AU ;
    dt:isPartOf C2004A04997:388 ;
    rdfs:comment "Schedule 12 Chinese originating goods - Abrievated Graph Key: S403"@en-AU ;
    skos:definition "Schedule 12 Chinese originating goods"@en-AU ;
    skos:narrower C2004A04997:388 ;
    skos:prefLabel "Schedule S403"@en-AU ;
    dcat:accessURL "https://www.legislation.gov.au/C2004A04997/2024-07-01/2024-07-01/text/1/epub/OEBPS/document_6/document_6.html#_Toc171755013"^^xsd:anyURI .

C2004A04997:404 a C2004A04997:Schedule ;
    rdfs:label "Schedule - S404 Schedule 13 Hong Kong originating goods"@en-AU ;
    dt:isPartOf C2004A04997:388 ;
    rdfs:comment "Schedule 13 Hong Kong originating goods - Abrievated Graph Key: S404"@en-AU ;
    skos:definition "Schedule 13 Hong Kong originating goods"@en-AU ;
    skos:narrower C2004A04997:388 ;
    skos:prefLabel "Schedule S404"@en-AU ;
    dcat:accessURL "https://www.legislation.gov.au/C2004A04997/2024-07-01/2024-07-01/text/1/epub/OEBPS/document_6/document_6.html#_Toc171755014"^^xsd:anyURI .

C2004A04997:405 a C2004A04997:Schedule ;
    rdfs:label "Schedule - S405 Schedule 14 Regional Comprehensive Economic Partnership RCEP originating goods"@en-AU ;
    dt:isPartOf C2004A04997:388 ;
    rdfs:comment "Schedule 14 Regional Comprehensive Economic Partnership RCEP originating goods - Abrievated Graph Key: S405"@en-AU ;
    skos:definition "Schedule 14 Regional Comprehensive Economic Partnership RCEP originating goods"@en-AU ;
    skos:narrower C2004A04997:388 ;
    skos:prefLabel "Schedule S405"@en-AU ;
    dcat:accessURL "https://www.legislation.gov.au/C2004A04997/2024-07-01/2024-07-01/text/1/epub/OEBPS/document_6/document_6.html#_Toc171755015"^^xsd:anyURI .

C2004A04997:406 a C2004A04997:Schedule ;
    rdfs:label "Schedule - S406 Schedule 15 UK originating goods"@en-AU ;
    dt:isPartOf C2004A04997:388 ;
    rdfs:comment "Schedule 15 UK originating goods - Abrievated Graph Key: S406"@en-AU ;
    skos:definition "Schedule 15 UK originating goods"@en-AU ;
    skos:narrower C2004A04997:388 ;
    skos:prefLabel "Schedule S406"@en-AU ;
    dcat:accessURL "https://www.legislation.gov.au/C2004A04997/2024-07-01/2024-07-01/text/1/epub/OEBPS/document_6/document_6.html#_Toc171755016"^^xsd:anyURI .

C2004A04997:407 a C2004A04997:Volume ;
    rdfs:label "Volume - V407 Volume 7"@en-AU ;
    dt:hasPart C2004A04997:408 ;
    rdfs:comment "Volume 7 - Abrievated Graph Key: V407"@en-AU ;
    skos:broader C2004A04997:408 ;
    skos:definition "Volume 7"@en-AU ;
    skos:prefLabel "Volume V407"@en-AU ;
    dcat:accessURL "https://www.legislation.gov.au/C2004A04997/2024-07-01/2024-07-01/text/1/epub/OEBPS/document_7/document_7.html"^^xsd:anyURI .

C2004A04997:409 a C2004A04997:Item ;
    rdfs:label "Item - I409 Endnote 1 About the endnotes"@en-AU ;
    dt:isPartOf C2004A04997:408 ;
    rdfs:comment "Endnote 1 About the endnotes - Abrievated Graph Key: I409"@en-AU ;
    skos:definition "Endnote 1 About the endnotes"@en-AU ;
    skos:narrower C2004A04997:408 ;
    skos:prefLabel "Item I409"@en-AU ;
    dcat:accessURL "https://www.legislation.gov.au/C2004A04997/2024-07-01/2024-07-01/text/1/epub/OEBPS/document_7/document_7.html#_Toc171755739"^^xsd:anyURI .

C2004A04997:41 a C2004A04997:Item ;
    rdfs:label "Item - I41 18  Calculation of concessional duty"@en-AU ;
    dt:isPartOf C2004A04997:36 ;
    rdfs:comment "18  Calculation of concessional duty - Abrievated Graph Key: I41"@en-AU ;
    skos:definition "18  Calculation of concessional duty"@en-AU ;
    skos:narrower C2004A04997:36 ;
    skos:prefLabel "Item I41"@en-AU ;
    dcat:accessURL "https://www.legislation.gov.au/C2004A04997/2024-07-01/2024-07-01/text/1/epub/OEBPS/document_1/document_1.html#_Toc172806541"^^xsd:anyURI .

C2004A04997:410 a C2004A04997:Item ;
    rdfs:label "Item - I410 Endnote 2 Abbreviation key"@en-AU ;
    dt:isPartOf C2004A04997:408 ;
    rdfs:comment "Endnote 2 Abbreviation key - Abrievated Graph Key: I410"@en-AU ;
    skos:definition "Endnote 2 Abbreviation key"@en-AU ;
    skos:narrower C2004A04997:408 ;
    skos:prefLabel "Item I410"@en-AU ;
    dcat:accessURL "https://www.legislation.gov.au/C2004A04997/2024-07-01/2024-07-01/text/1/epub/OEBPS/document_7/document_7.html#_Toc171755740"^^xsd:anyURI .

C2004A04997:411 a C2004A04997:Item ;
    rdfs:label "Item - I411 Endnote 3 Legislation history"@en-AU ;
    dt:isPartOf C2004A04997:408 ;
    rdfs:comment "Endnote 3 Legislation history - Abrievated Graph Key: I411"@en-AU ;
    skos:definition "Endnote 3 Legislation history"@en-AU ;
    skos:narrower C2004A04997:408 ;
    skos:prefLabel "Item I411"@en-AU ;
    dcat:accessURL "https://www.legislation.gov.au/C2004A04997/2024-07-01/2024-07-01/text/1/epub/OEBPS/document_7/document_7.html#_Toc171755741"^^xsd:anyURI .

C2004A04997:412 a C2004A04997:Item ;
    rdfs:label "Item - I412 Endnote 4 Amendment history"@en-AU ;
    dt:isPartOf C2004A04997:408 ;
    rdfs:comment "Endnote 4 Amendment history - Abrievated Graph Key: I412"@en-AU ;
    skos:definition "Endnote 4 Amendment history"@en-AU ;
    skos:narrower C2004A04997:408 ;
    skos:prefLabel "Item I412"@en-AU ;
    dcat:accessURL "https://www.legislation.gov.au/C2004A04997/2024-07-01/2024-07-01/text/1/epub/OEBPS/document_7/document_7.html#_Toc171755742"^^xsd:anyURI .

C2004A04997:42 a C2004A04997:Item ;
    rdfs:label "Item - I42 18 A  Temporary increase in duties for goods from Russia or Belarus"@en-AU ;
    dt:isPartOf C2004A04997:36 ;
    rdfs:comment "18 A  Temporary increase in duties for goods from Russia or Belarus - Abrievated Graph Key: I42"@en-AU ;
    skos:definition "18 A  Temporary increase in duties for goods from Russia or Belarus"@en-AU ;
    skos:narrower C2004A04997:36 ;
    skos:prefLabel "Item I42"@en-AU ;
    dcat:accessURL "https://www.legislation.gov.au/C2004A04997/2024-07-01/2024-07-01/text/1/epub/OEBPS/document_1/document_1.html#_Toc172806542"^^xsd:anyURI .

C2004A04997:43 a C2004A04997:Item ;
    rdfs:label "Item - I43 18 B  Temporary decrease in duties for goods from Ukraine"@en-AU ;
    dt:isPartOf C2004A04997:36 ;
    rdfs:comment "18 B  Temporary decrease in duties for goods from Ukraine - Abrievated Graph Key: I43"@en-AU ;
    skos:definition "18 B  Temporary decrease in duties for goods from Ukraine"@en-AU ;
    skos:narrower C2004A04997:36 ;
    skos:prefLabel "Item I43"@en-AU ;
    dcat:accessURL "https://www.legislation.gov.au/C2004A04997/2024-07-01/2024-07-01/text/1/epub/OEBPS/document_1/document_1.html#_Toc172806543"^^xsd:anyURI .

C2004A04997:44 a C2004A04997:Item ;
    rdfs:label "Item - I44 19  Indexation of CPI indexed rates"@en-AU ;
    dt:isPartOf C2004A04997:36 ;
    rdfs:comment "19  Indexation of CPI indexed rates - Abrievated Graph Key: I44"@en-AU ;
    skos:definition "19  Indexation of CPI indexed rates"@en-AU ;
    skos:narrower C2004A04997:36 ;
    skos:prefLabel "Item I44"@en-AU ;
    dcat:accessURL "https://www.legislation.gov.au/C2004A04997/2024-07-01/2024-07-01/text/1/epub/OEBPS/document_1/document_1.html#_Toc172806544"^^xsd:anyURI .

C2004A04997:45 a C2004A04997:Item ;
    rdfs:label "Item - I45 19 AAA  Rounding of fuel duty rates"@en-AU ;
    dt:isPartOf C2004A04997:36 ;
    rdfs:comment "19 AAA  Rounding of fuel duty rates - Abrievated Graph Key: I45"@en-AU ;
    skos:definition "19 AAA  Rounding of fuel duty rates"@en-AU ;
    skos:narrower C2004A04997:36 ;
    skos:prefLabel "Item I45"@en-AU ;
    dcat:accessURL "https://www.legislation.gov.au/C2004A04997/2024-07-01/2024-07-01/text/1/epub/OEBPS/document_1/document_1.html#_Toc172806545"^^xsd:anyURI .

C2004A04997:46 a C2004A04997:Item ;
    rdfs:label "Item - I46 19 AAB  Change in fuel duty rates"@en-AU ;
    dt:isPartOf C2004A04997:36 ;
    rdfs:comment "19 AAB  Change in fuel duty rates - Abrievated Graph Key: I46"@en-AU ;
    skos:definition "19 AAB  Change in fuel duty rates"@en-AU ;
    skos:narrower C2004A04997:36 ;
    skos:prefLabel "Item I46"@en-AU ;
    dcat:accessURL "https://www.legislation.gov.au/C2004A04997/2024-07-01/2024-07-01/text/1/epub/OEBPS/document_1/document_1.html#_Toc172806546"^^xsd:anyURI .

C2004A04997:47 a C2004A04997:Item ;
    rdfs:label "Item - I47 19 AABA  Temporary reduction in indexed fuel duty rates"@en-AU ;
    dt:isPartOf C2004A04997:36 ;
    rdfs:comment "19 AABA  Temporary reduction in indexed fuel duty rates - Abrievated Graph Key: I47"@en-AU ;
    skos:definition "19 AABA  Temporary reduction in indexed fuel duty rates"@en-AU ;
    skos:narrower C2004A04997:36 ;
    skos:prefLabel "Item I47"@en-AU ;
    dcat:accessURL "https://www.legislation.gov.au/C2004A04997/2024-07-01/2024-07-01/text/1/epub/OEBPS/document_1/document_1.html#_Toc172806547"^^xsd:anyURI .

C2004A04997:48 a C2004A04997:Item ;
    rdfs:label "Item - I48 19 AABB  Temporary reduction in other duty rates"@en-AU ;
    dt:isPartOf C2004A04997:36 ;
    rdfs:comment "19 AABB  Temporary reduction in other duty rates - Abrievated Graph Key: I48"@en-AU ;
    skos:definition "19 AABB  Temporary reduction in other duty rates"@en-AU ;
    skos:narrower C2004A04997:36 ;
    skos:prefLabel "Item I48"@en-AU ;
    dcat:accessURL "https://www.legislation.gov.au/C2004A04997/2024-07-01/2024-07-01/text/1/epub/OEBPS/document_1/document_1.html#_Toc172806548"^^xsd:anyURI .

C2004A04997:49 a C2004A04997:Item ;
    rdfs:label "Item - I49 19 AAC  Fuel duty rates"@en-AU ;
    dt:isPartOf C2004A04997:36 ;
    rdfs:comment "19 AAC  Fuel duty rates - Abrievated Graph Key: I49"@en-AU ;
    skos:definition "19 AAC  Fuel duty rates"@en-AU ;
    skos:narrower C2004A04997:36 ;
    skos:prefLabel "Item I49"@en-AU ;
    dcat:accessURL "https://www.legislation.gov.au/C2004A04997/2024-07-01/2024-07-01/text/1/epub/OEBPS/document_1/document_1.html#_Toc172806549"^^xsd:anyURI .

C2004A04997:5 a C2004A04997:Item ;
    rdfs:label "Item - I5 3  Definitions"@en-AU ;
    dt:isPartOf C2004A04997:2 ;
    rdfs:comment "3  Definitions - Abrievated Graph Key: I5"@en-AU ;
    skos:definition "3  Definitions"@en-AU ;
    skos:narrower C2004A04997:2 ;
    skos:prefLabel "Item I5"@en-AU ;
    dcat:accessURL "https://www.legislation.gov.au/C2004A04997/2024-07-01/2024-07-01/text/1/epub/OEBPS/document_1/document_1.html#_Toc172806505"^^xsd:anyURI .

C2004A04997:50 a C2004A04997:Item ;
    rdfs:label "Item - I50 19 AA  Alcohol duty rates"@en-AU ;
    dt:isPartOf C2004A04997:36 ;
    rdfs:comment "19 AA  Alcohol duty rates - Abrievated Graph Key: I50"@en-AU ;
    skos:definition "19 AA  Alcohol duty rates"@en-AU ;
    skos:narrower C2004A04997:36 ;
    skos:prefLabel "Item I50"@en-AU ;
    dcat:accessURL "https://www.legislation.gov.au/C2004A04997/2024-07-01/2024-07-01/text/1/epub/OEBPS/document_1/document_1.html#_Toc172806550"^^xsd:anyURI .

C2004A04997:51 a C2004A04997:Item ;
    rdfs:label "Item - I51 19 AB  Indexation of tobacco duty rates"@en-AU ;
    dt:isPartOf C2004A04997:36 ;
    rdfs:comment "19 AB  Indexation of tobacco duty rates - Abrievated Graph Key: I51"@en-AU ;
    skos:definition "19 AB  Indexation of tobacco duty rates"@en-AU ;
    skos:narrower C2004A04997:36 ;
    skos:prefLabel "Item I51"@en-AU ;
    dcat:accessURL "https://www.legislation.gov.au/C2004A04997/2024-07-01/2024-07-01/text/1/epub/OEBPS/document_1/document_1.html#_Toc172806551"^^xsd:anyURI .

C2004A04997:52 a C2004A04997:Item ;
    rdfs:label "Item - I52 19 AC  List of tobacco duty rates to be indexed under section 19 AB"@en-AU ;
    dt:isPartOf C2004A04997:36 ;
    rdfs:comment "19 AC  List of tobacco duty rates to be indexed under section 19 AB - Abrievated Graph Key: I52"@en-AU ;
    skos:definition "19 AC  List of tobacco duty rates to be indexed under section 19 AB"@en-AU ;
    skos:narrower C2004A04997:36 ;
    skos:prefLabel "Item I52"@en-AU ;
    dcat:accessURL "https://www.legislation.gov.au/C2004A04997/2024-07-01/2024-07-01/text/1/epub/OEBPS/document_1/document_1.html#_Toc172806552"^^xsd:anyURI .

C2004A04997:53 a C2004A04997:Item ;
    rdfs:label "Item - I53 19 ACA  Other tobacco duty rates"@en-AU ;
    dt:isPartOf C2004A04997:36 ;
    rdfs:comment "19 ACA  Other tobacco duty rates - Abrievated Graph Key: I53"@en-AU ;
    skos:definition "19 ACA  Other tobacco duty rates"@en-AU ;
    skos:narrower C2004A04997:36 ;
    skos:prefLabel "Item I53"@en-AU ;
    dcat:accessURL "https://www.legislation.gov.au/C2004A04997/2024-07-01/2024-07-01/text/1/epub/OEBPS/document_1/document_1.html#_Toc172806553"^^xsd:anyURI .

C2004A04997:54 a C2004A04997:Item ;
    rdfs:label "Item - I54 19 AD  Change in duty rate of certain liquefied petroleum gases liquefied natural gases and compressed natural gases"@en-AU ;
    dt:isPartOf C2004A04997:36 ;
    rdfs:comment "19 AD  Change in duty rate of certain liquefied petroleum gases liquefied natural gases and compressed natural gases - Abrievated Graph Key: I54"@en-AU ;
    skos:definition "19 AD  Change in duty rate of certain liquefied petroleum gases liquefied natural gases and compressed natural gases"@en-AU ;
    skos:narrower C2004A04997:36 ;
    skos:prefLabel "Item I54"@en-AU ;
    dcat:accessURL "https://www.legislation.gov.au/C2004A04997/2024-07-01/2024-07-01/text/1/epub/OEBPS/document_1/document_1.html#_Toc172806554"^^xsd:anyURI .

C2004A04997:55 a C2004A04997:Item ;
    rdfs:label "Item - I55 20  Duty where goods consist of certain containers and certain contents"@en-AU ;
    dt:isPartOf C2004A04997:36 ;
    rdfs:comment "20  Duty where goods consist of certain containers and certain contents - Abrievated Graph Key: I55"@en-AU ;
    skos:definition "20  Duty where goods consist of certain containers and certain contents"@en-AU ;
    skos:narrower C2004A04997:36 ;
    skos:prefLabel "Item I55"@en-AU ;
    dcat:accessURL "https://www.legislation.gov.au/C2004A04997/2024-07-01/2024-07-01/text/1/epub/OEBPS/document_1/document_1.html#_Toc172806555"^^xsd:anyURI .

C2004A04997:57 a C2004A04997:Item ;
    rdfs:label "Item - I57 20 A  Regulations"@en-AU ;
    dt:isPartOf C2004A04997:56 ;
    rdfs:comment "20 A  Regulations - Abrievated Graph Key: I57"@en-AU ;
    skos:definition "20 A  Regulations"@en-AU ;
    skos:narrower C2004A04997:56 ;
    skos:prefLabel "Item I57"@en-AU ;
    dcat:accessURL "https://www.legislation.gov.au/C2004A04997/2024-07-01/2024-07-01/text/1/epub/OEBPS/document_1/document_1.html#_Toc172806557"^^xsd:anyURI .

C2004A04997:58 a C2004A04997:Item ;
    rdfs:label "Item - I58 21  Repeal of the Customs Tariff Act 1987 etc"@en-AU ;
    dt:isPartOf C2004A04997:56 ;
    rdfs:comment "21  Repeal of the Customs Tariff Act 1987 etc - Abrievated Graph Key: I58"@en-AU ;
    skos:definition "21  Repeal of the Customs Tariff Act 1987 etc"@en-AU ;
    skos:narrower C2004A04997:56 ;
    skos:prefLabel "Item I58"@en-AU ;
    dcat:accessURL "https://www.legislation.gov.au/C2004A04997/2024-07-01/2024-07-01/text/1/epub/OEBPS/document_1/document_1.html#_Toc172806558"^^xsd:anyURI .

C2004A04997:59 a C2004A04997:Item ;
    rdfs:label "Item - I59 22  Transitional"@en-AU ;
    dt:isPartOf C2004A04997:56 ;
    rdfs:comment "22  Transitional - Abrievated Graph Key: I59"@en-AU ;
    skos:definition "22  Transitional"@en-AU ;
    skos:narrower C2004A04997:56 ;
    skos:prefLabel "Item I59"@en-AU ;
    dcat:accessURL "https://www.legislation.gov.au/C2004A04997/2024-07-01/2024-07-01/text/1/epub/OEBPS/document_1/document_1.html#_Toc172806559"^^xsd:anyURI .

C2004A04997:6 a C2004A04997:Item ;
    rdfs:label "Item - I6 3 A  Act does not extend to Norfolk Island"@en-AU ;
    dt:isPartOf C2004A04997:2 ;
    rdfs:comment "3 A  Act does not extend to Norfolk Island - Abrievated Graph Key: I6"@en-AU ;
    skos:definition "3 A  Act does not extend to Norfolk Island"@en-AU ;
    skos:narrower C2004A04997:2 ;
    skos:prefLabel "Item I6"@en-AU ;
    dcat:accessURL "https://www.legislation.gov.au/C2004A04997/2024-07-01/2024-07-01/text/1/epub/OEBPS/document_1/document_1.html#_Toc172806506"^^xsd:anyURI .

C2004A04997:60 a C2004A04997:Schedule ;
    rdfs:label "Schedule - S60 Schedule 2 General rules for the interpretation of Schedule 3"@en-AU ;
    dt:isPartOf C2004A04997:1 ;
    rdfs:comment "Schedule 2 General rules for the interpretation of Schedule 3 - Abrievated Graph Key: S60"@en-AU ;
    skos:definition "Schedule 2 General rules for the interpretation of Schedule 3"@en-AU ;
    skos:narrower C2004A04997:1 ;
    skos:prefLabel "Schedule S60"@en-AU ;
    dcat:accessURL "https://www.legislation.gov.au/C2004A04997/2024-07-01/2024-07-01/text/1/epub/OEBPS/document_1/document_1.html#_Toc172806560"^^xsd:anyURI .

C2004A04997:63 a C2004A04997:Item ;
    rdfs:label "Item - I63 Notes"@en-AU ;
    dt:isPartOf C2004A04997:62 ;
    rdfs:comment "Notes - Abrievated Graph Key: I63"@en-AU ;
    skos:definition "Notes"@en-AU ;
    skos:narrower C2004A04997:62 ;
    skos:prefLabel "Item I63"@en-AU ;
    dcat:accessURL "https://www.legislation.gov.au/C2004A04997/2024-07-01/2024-07-01/text/1/epub/OEBPS/document_1/document_1.html#_Toc172806563"^^xsd:anyURI .

C2004A04997:64 a C2004A04997:Chapter ;
    rdfs:label "Chapter - C64 Chapter 1 Live animals"@en-AU ;
    dt:isPartOf C2004A04997:62 ;
    rdfs:comment "Chapter 1 Live animals - Abrievated Graph Key: C64"@en-AU ;
    skos:definition "Chapter 1 Live animals"@en-AU ;
    skos:narrower C2004A04997:62 ;
    skos:prefLabel "Chapter C64"@en-AU ;
    dcat:accessURL "https://www.legislation.gov.au/C2004A04997/2024-07-01/2024-07-01/text/1/epub/OEBPS/document_1/document_1.html#_Toc172806564"^^xsd:anyURI .

C2004A04997:65 a C2004A04997:Item ;
    rdfs:label "Item - I65 Note"@en-AU ;
    dt:isPartOf C2004A04997:62 ;
    rdfs:comment "Note - Abrievated Graph Key: I65"@en-AU ;
    skos:definition "Note"@en-AU ;
    skos:narrower C2004A04997:62 ;
    skos:prefLabel "Item I65"@en-AU ;
    dcat:accessURL "https://www.legislation.gov.au/C2004A04997/2024-07-01/2024-07-01/text/1/epub/OEBPS/document_1/document_1.html#_Toc172806565"^^xsd:anyURI .

C2004A04997:66 a C2004A04997:Chapter ;
    rdfs:label "Chapter - C66 Chapter 2 Meat and edible meat offal"@en-AU ;
    dt:isPartOf C2004A04997:62 ;
    rdfs:comment "Chapter 2 Meat and edible meat offal - Abrievated Graph Key: C66"@en-AU ;
    skos:definition "Chapter 2 Meat and edible meat offal"@en-AU ;
    skos:narrower C2004A04997:62 ;
    skos:prefLabel "Chapter C66"@en-AU ;
    dcat:accessURL "https://www.legislation.gov.au/C2004A04997/2024-07-01/2024-07-01/text/1/epub/OEBPS/document_1/document_1.html#_Toc172806566"^^xsd:anyURI .

C2004A04997:67 a C2004A04997:Item ;
    rdfs:label "Item - I67 Note"@en-AU ;
    dt:isPartOf C2004A04997:62 ;
    rdfs:comment "Note - Abrievated Graph Key: I67"@en-AU ;
    skos:definition "Note"@en-AU ;
    skos:narrower C2004A04997:62 ;
    skos:prefLabel "Item I67"@en-AU ;
    dcat:accessURL "https://www.legislation.gov.au/C2004A04997/2024-07-01/2024-07-01/text/1/epub/OEBPS/document_1/document_1.html#_Toc172806567"^^xsd:anyURI .

C2004A04997:68 a C2004A04997:Chapter ;
    rdfs:label "Chapter - C68 Chapter 3 Fish and crustaceans molluscs and other aquatic invertebrates"@en-AU ;
    dt:isPartOf C2004A04997:62 ;
    rdfs:comment "Chapter 3 Fish and crustaceans molluscs and other aquatic invertebrates - Abrievated Graph Key: C68"@en-AU ;
    skos:definition "Chapter 3 Fish and crustaceans molluscs and other aquatic invertebrates"@en-AU ;
    skos:narrower C2004A04997:62 ;
    skos:prefLabel "Chapter C68"@en-AU ;
    dcat:accessURL "https://www.legislation.gov.au/C2004A04997/2024-07-01/2024-07-01/text/1/epub/OEBPS/document_1/document_1.html#_Toc172806568"^^xsd:anyURI .

C2004A04997:69 a C2004A04997:Item ;
    rdfs:label "Item - I69 Notes"@en-AU ;
    dt:isPartOf C2004A04997:62 ;
    rdfs:comment "Notes - Abrievated Graph Key: I69"@en-AU ;
    skos:definition "Notes"@en-AU ;
    skos:narrower C2004A04997:62 ;
    skos:prefLabel "Item I69"@en-AU ;
    dcat:accessURL "https://www.legislation.gov.au/C2004A04997/2024-07-01/2024-07-01/text/1/epub/OEBPS/document_1/document_1.html#_Toc172806569"^^xsd:anyURI .

C2004A04997:7 a C2004A04997:Item ;
    rdfs:label "Item - I7 4  Headings in Schedule 3"@en-AU ;
    dt:isPartOf C2004A04997:2 ;
    rdfs:comment "4  Headings in Schedule 3 - Abrievated Graph Key: I7"@en-AU ;
    skos:definition "4  Headings in Schedule 3"@en-AU ;
    skos:narrower C2004A04997:2 ;
    skos:prefLabel "Item I7"@en-AU ;
    dcat:accessURL "https://www.legislation.gov.au/C2004A04997/2024-07-01/2024-07-01/text/1/epub/OEBPS/document_1/document_1.html#_Toc172806507"^^xsd:anyURI .

C2004A04997:70 a C2004A04997:Chapter ;
    rdfs:label "Chapter - C70 Chapter 4 Dairy produce birds eggs natural honey edible products of animal origin not elsewhere specified or included"@en-AU ;
    dt:isPartOf C2004A04997:62 ;
    rdfs:comment "Chapter 4 Dairy produce birds eggs natural honey edible products of animal origin not elsewhere specified or included - Abrievated Graph Key: C70"@en-AU ;
    skos:definition "Chapter 4 Dairy produce birds eggs natural honey edible products of animal origin not elsewhere specified or included"@en-AU ;
    skos:narrower C2004A04997:62 ;
    skos:prefLabel "Chapter C70"@en-AU ;
    dcat:accessURL "https://www.legislation.gov.au/C2004A04997/2024-07-01/2024-07-01/text/1/epub/OEBPS/document_1/document_1.html#_Toc172806570"^^xsd:anyURI .

C2004A04997:71 a C2004A04997:Item ;
    rdfs:label "Item - I71 Notes"@en-AU ;
    dt:isPartOf C2004A04997:62 ;
    rdfs:comment "Notes - Abrievated Graph Key: I71"@en-AU ;
    skos:definition "Notes"@en-AU ;
    skos:narrower C2004A04997:62 ;
    skos:prefLabel "Item I71"@en-AU ;
    dcat:accessURL "https://www.legislation.gov.au/C2004A04997/2024-07-01/2024-07-01/text/1/epub/OEBPS/document_1/document_1.html#_Toc172806571"^^xsd:anyURI .

C2004A04997:72 a C2004A04997:Item ;
    rdfs:label "Item - I72 Subheading Notes"@en-AU ;
    dt:isPartOf C2004A04997:62 ;
    rdfs:comment "Subheading Notes - Abrievated Graph Key: I72"@en-AU ;
    skos:definition "Subheading Notes"@en-AU ;
    skos:narrower C2004A04997:62 ;
    skos:prefLabel "Item I72"@en-AU ;
    dcat:accessURL "https://www.legislation.gov.au/C2004A04997/2024-07-01/2024-07-01/text/1/epub/OEBPS/document_1/document_1.html#_Toc172806572"^^xsd:anyURI .

C2004A04997:73 a C2004A04997:Chapter ;
    rdfs:label "Chapter - C73 Chapter 5 Products of animal origin not elsewhere specified or included"@en-AU ;
    dt:isPartOf C2004A04997:62 ;
    rdfs:comment "Chapter 5 Products of animal origin not elsewhere specified or included - Abrievated Graph Key: C73"@en-AU ;
    skos:definition "Chapter 5 Products of animal origin not elsewhere specified or included"@en-AU ;
    skos:narrower C2004A04997:62 ;
    skos:prefLabel "Chapter C73"@en-AU ;
    dcat:accessURL "https://www.legislation.gov.au/C2004A04997/2024-07-01/2024-07-01/text/1/epub/OEBPS/document_1/document_1.html#_Toc172806573"^^xsd:anyURI .

C2004A04997:74 a C2004A04997:Item ;
    rdfs:label "Item - I74 Notes"@en-AU ;
    dt:isPartOf C2004A04997:62 ;
    rdfs:comment "Notes - Abrievated Graph Key: I74"@en-AU ;
    skos:definition "Notes"@en-AU ;
    skos:narrower C2004A04997:62 ;
    skos:prefLabel "Item I74"@en-AU ;
    dcat:accessURL "https://www.legislation.gov.au/C2004A04997/2024-07-01/2024-07-01/text/1/epub/OEBPS/document_1/document_1.html#_Toc172806574"^^xsd:anyURI .

C2004A04997:75 a C2004A04997:Section ;
    rdfs:label "Section - S75 Section IIVegetable products"@en-AU ;
    dt:isPartOf C2004A04997:61 ;
    rdfs:comment "Section IIVegetable products - Abrievated Graph Key: S75"@en-AU ;
    skos:definition "Section IIVegetable products"@en-AU ;
    skos:narrower C2004A04997:61 ;
    skos:prefLabel "Section S75"@en-AU ;
    dcat:accessURL "https://www.legislation.gov.au/C2004A04997/2024-07-01/2024-07-01/text/1/epub/OEBPS/document_1/document_1.html#_Toc172806575"^^xsd:anyURI .

C2004A04997:76 a C2004A04997:Item ;
    rdfs:label "Item - I76 Note"@en-AU ;
    dt:isPartOf C2004A04997:61 ;
    rdfs:comment "Note - Abrievated Graph Key: I76"@en-AU ;
    skos:definition "Note"@en-AU ;
    skos:narrower C2004A04997:61 ;
    skos:prefLabel "Item I76"@en-AU ;
    dcat:accessURL "https://www.legislation.gov.au/C2004A04997/2024-07-01/2024-07-01/text/1/epub/OEBPS/document_1/document_1.html#_Toc172806576"^^xsd:anyURI .

C2004A04997:77 a C2004A04997:Chapter ;
    rdfs:label "Chapter - C77 Chapter 6 Live trees and other plants bulbs roots and the like cut flowers and ornamental foliage"@en-AU ;
    dt:isPartOf C2004A04997:61 ;
    rdfs:comment "Chapter 6 Live trees and other plants bulbs roots and the like cut flowers and ornamental foliage - Abrievated Graph Key: C77"@en-AU ;
    skos:definition "Chapter 6 Live trees and other plants bulbs roots and the like cut flowers and ornamental foliage"@en-AU ;
    skos:narrower C2004A04997:61 ;
    skos:prefLabel "Chapter C77"@en-AU ;
    dcat:accessURL "https://www.legislation.gov.au/C2004A04997/2024-07-01/2024-07-01/text/1/epub/OEBPS/document_1/document_1.html#_Toc172806577"^^xsd:anyURI .

C2004A04997:78 a C2004A04997:Item ;
    rdfs:label "Item - I78 Notes"@en-AU ;
    dt:isPartOf C2004A04997:61 ;
    rdfs:comment "Notes - Abrievated Graph Key: I78"@en-AU ;
    skos:definition "Notes"@en-AU ;
    skos:narrower C2004A04997:61 ;
    skos:prefLabel "Item I78"@en-AU ;
    dcat:accessURL "https://www.legislation.gov.au/C2004A04997/2024-07-01/2024-07-01/text/1/epub/OEBPS/document_1/document_1.html#_Toc172806578"^^xsd:anyURI .

C2004A04997:79 a C2004A04997:Chapter ;
    rdfs:label "Chapter - C79 Chapter 7 Edible vegetables and certain roots and tubers"@en-AU ;
    dt:isPartOf C2004A04997:61 ;
    rdfs:comment "Chapter 7 Edible vegetables and certain roots and tubers - Abrievated Graph Key: C79"@en-AU ;
    skos:definition "Chapter 7 Edible vegetables and certain roots and tubers"@en-AU ;
    skos:narrower C2004A04997:61 ;
    skos:prefLabel "Chapter C79"@en-AU ;
    dcat:accessURL "https://www.legislation.gov.au/C2004A04997/2024-07-01/2024-07-01/text/1/epub/OEBPS/document_1/document_1.html#_Toc172806579"^^xsd:anyURI .

C2004A04997:8 a C2004A04997:Item ;
    rdfs:label "Item - I8 5  Items in Schedule 4"@en-AU ;
    dt:isPartOf C2004A04997:2 ;
    rdfs:comment "5  Items in Schedule 4 - Abrievated Graph Key: I8"@en-AU ;
    skos:definition "5  Items in Schedule 4"@en-AU ;
    skos:narrower C2004A04997:2 ;
    skos:prefLabel "Item I8"@en-AU ;
    dcat:accessURL "https://www.legislation.gov.au/C2004A04997/2024-07-01/2024-07-01/text/1/epub/OEBPS/document_1/document_1.html#_Toc172806508"^^xsd:anyURI .

C2004A04997:80 a C2004A04997:Item ;
    rdfs:label "Item - I80 Notes"@en-AU ;
    dt:isPartOf C2004A04997:61 ;
    rdfs:comment "Notes - Abrievated Graph Key: I80"@en-AU ;
    skos:definition "Notes"@en-AU ;
    skos:narrower C2004A04997:61 ;
    skos:prefLabel "Item I80"@en-AU ;
    dcat:accessURL "https://www.legislation.gov.au/C2004A04997/2024-07-01/2024-07-01/text/1/epub/OEBPS/document_1/document_1.html#_Toc172806580"^^xsd:anyURI .

C2004A04997:81 a C2004A04997:Chapter ;
    rdfs:label "Chapter - C81 Chapter 8 Edible fruit and nuts peel of citrus fruit or melons"@en-AU ;
    dt:isPartOf C2004A04997:61 ;
    rdfs:comment "Chapter 8 Edible fruit and nuts peel of citrus fruit or melons - Abrievated Graph Key: C81"@en-AU ;
    skos:definition "Chapter 8 Edible fruit and nuts peel of citrus fruit or melons"@en-AU ;
    skos:narrower C2004A04997:61 ;
    skos:prefLabel "Chapter C81"@en-AU ;
    dcat:accessURL "https://www.legislation.gov.au/C2004A04997/2024-07-01/2024-07-01/text/1/epub/OEBPS/document_1/document_1.html#_Toc172806581"^^xsd:anyURI .

C2004A04997:82 a C2004A04997:Item ;
    rdfs:label "Item - I82 Notes"@en-AU ;
    dt:isPartOf C2004A04997:61 ;
    rdfs:comment "Notes - Abrievated Graph Key: I82"@en-AU ;
    skos:definition "Notes"@en-AU ;
    skos:narrower C2004A04997:61 ;
    skos:prefLabel "Item I82"@en-AU ;
    dcat:accessURL "https://www.legislation.gov.au/C2004A04997/2024-07-01/2024-07-01/text/1/epub/OEBPS/document_1/document_1.html#_Toc172806582"^^xsd:anyURI .

C2004A04997:83 a C2004A04997:Chapter ;
    rdfs:label "Chapter - C83 Chapter 9 Coffee tea mate and spices"@en-AU ;
    dt:isPartOf C2004A04997:61 ;
    rdfs:comment "Chapter 9 Coffee tea mate and spices - Abrievated Graph Key: C83"@en-AU ;
    skos:definition "Chapter 9 Coffee tea mate and spices"@en-AU ;
    skos:narrower C2004A04997:61 ;
    skos:prefLabel "Chapter C83"@en-AU ;
    dcat:accessURL "https://www.legislation.gov.au/C2004A04997/2024-07-01/2024-07-01/text/1/epub/OEBPS/document_1/document_1.html#_Toc172806583"^^xsd:anyURI .

C2004A04997:84 a C2004A04997:Item ;
    rdfs:label "Item - I84 Notes"@en-AU ;
    dt:isPartOf C2004A04997:61 ;
    rdfs:comment "Notes - Abrievated Graph Key: I84"@en-AU ;
    skos:definition "Notes"@en-AU ;
    skos:narrower C2004A04997:61 ;
    skos:prefLabel "Item I84"@en-AU ;
    dcat:accessURL "https://www.legislation.gov.au/C2004A04997/2024-07-01/2024-07-01/text/1/epub/OEBPS/document_1/document_1.html#_Toc172806584"^^xsd:anyURI .

C2004A04997:85 a C2004A04997:Chapter ;
    rdfs:label "Chapter - C85 Chapter 10 Cereals"@en-AU ;
    dt:isPartOf C2004A04997:61 ;
    rdfs:comment "Chapter 10 Cereals - Abrievated Graph Key: C85"@en-AU ;
    skos:definition "Chapter 10 Cereals"@en-AU ;
    skos:narrower C2004A04997:61 ;
    skos:prefLabel "Chapter C85"@en-AU ;
    dcat:accessURL "https://www.legislation.gov.au/C2004A04997/2024-07-01/2024-07-01/text/1/epub/OEBPS/document_1/document_1.html#_Toc172806585"^^xsd:anyURI .

C2004A04997:86 a C2004A04997:Item ;
    rdfs:label "Item - I86 Notes"@en-AU ;
    dt:isPartOf C2004A04997:61 ;
    rdfs:comment "Notes - Abrievated Graph Key: I86"@en-AU ;
    skos:definition "Notes"@en-AU ;
    skos:narrower C2004A04997:61 ;
    skos:prefLabel "Item I86"@en-AU ;
    dcat:accessURL "https://www.legislation.gov.au/C2004A04997/2024-07-01/2024-07-01/text/1/epub/OEBPS/document_1/document_1.html#_Toc172806586"^^xsd:anyURI .

C2004A04997:87 a C2004A04997:Item ;
    rdfs:label "Item - I87 Subheading Note"@en-AU ;
    dt:isPartOf C2004A04997:61 ;
    rdfs:comment "Subheading Note - Abrievated Graph Key: I87"@en-AU ;
    skos:definition "Subheading Note"@en-AU ;
    skos:narrower C2004A04997:61 ;
    skos:prefLabel "Item I87"@en-AU ;
    dcat:accessURL "https://www.legislation.gov.au/C2004A04997/2024-07-01/2024-07-01/text/1/epub/OEBPS/document_1/document_1.html#_Toc172806587"^^xsd:anyURI .

C2004A04997:88 a C2004A04997:Chapter ;
    rdfs:label "Chapter - C88 Chapter 11 Products of the milling industry malt starches inulin wheat gluten"@en-AU ;
    dt:isPartOf C2004A04997:61 ;
    rdfs:comment "Chapter 11 Products of the milling industry malt starches inulin wheat gluten - Abrievated Graph Key: C88"@en-AU ;
    skos:definition "Chapter 11 Products of the milling industry malt starches inulin wheat gluten"@en-AU ;
    skos:narrower C2004A04997:61 ;
    skos:prefLabel "Chapter C88"@en-AU ;
    dcat:accessURL "https://www.legislation.gov.au/C2004A04997/2024-07-01/2024-07-01/text/1/epub/OEBPS/document_1/document_1.html#_Toc172806588"^^xsd:anyURI .

C2004A04997:89 a C2004A04997:Item ;
    rdfs:label "Item - I89 Notes"@en-AU ;
    dt:isPartOf C2004A04997:61 ;
    rdfs:comment "Notes - Abrievated Graph Key: I89"@en-AU ;
    skos:definition "Notes"@en-AU ;
    skos:narrower C2004A04997:61 ;
    skos:prefLabel "Item I89"@en-AU ;
    dcat:accessURL "https://www.legislation.gov.au/C2004A04997/2024-07-01/2024-07-01/text/1/epub/OEBPS/document_1/document_1.html#_Toc172806589"^^xsd:anyURI .

C2004A04997:9 a C2004A04997:Item ;
    rdfs:label "Item - I9 6  Tariff classification"@en-AU ;
    dt:isPartOf C2004A04997:2 ;
    rdfs:comment "6  Tariff classification - Abrievated Graph Key: I9"@en-AU ;
    skos:definition "6  Tariff classification"@en-AU ;
    skos:narrower C2004A04997:2 ;
    skos:prefLabel "Item I9"@en-AU ;
    dcat:accessURL "https://www.legislation.gov.au/C2004A04997/2024-07-01/2024-07-01/text/1/epub/OEBPS/document_1/document_1.html#_Toc172806509"^^xsd:anyURI .

C2004A04997:90 a C2004A04997:Chapter ;
    rdfs:label "Chapter - C90 Chapter 12 Oil seeds and oleaginous fruits miscellaneous grains seeds and fruit industrial or medicinal plants straw and fodder"@en-AU ;
    dt:isPartOf C2004A04997:61 ;
    rdfs:comment "Chapter 12 Oil seeds and oleaginous fruits miscellaneous grains seeds and fruit industrial or medicinal plants straw and fodder - Abrievated Graph Key: C90"@en-AU ;
    skos:definition "Chapter 12 Oil seeds and oleaginous fruits miscellaneous grains seeds and fruit industrial or medicinal plants straw and fodder"@en-AU ;
    skos:narrower C2004A04997:61 ;
    skos:prefLabel "Chapter C90"@en-AU ;
    dcat:accessURL "https://www.legislation.gov.au/C2004A04997/2024-07-01/2024-07-01/text/1/epub/OEBPS/document_1/document_1.html#_Toc172806590"^^xsd:anyURI .

C2004A04997:91 a C2004A04997:Item ;
    rdfs:label "Item - I91 Notes"@en-AU ;
    dt:isPartOf C2004A04997:61 ;
    rdfs:comment "Notes - Abrievated Graph Key: I91"@en-AU ;
    skos:definition "Notes"@en-AU ;
    skos:narrower C2004A04997:61 ;
    skos:prefLabel "Item I91"@en-AU ;
    dcat:accessURL "https://www.legislation.gov.au/C2004A04997/2024-07-01/2024-07-01/text/1/epub/OEBPS/document_1/document_1.html#_Toc172806591"^^xsd:anyURI .

C2004A04997:92 a C2004A04997:Item ;
    rdfs:label "Item - I92 Subheading Note"@en-AU ;
    dt:isPartOf C2004A04997:61 ;
    rdfs:comment "Subheading Note - Abrievated Graph Key: I92"@en-AU ;
    skos:definition "Subheading Note"@en-AU ;
    skos:narrower C2004A04997:61 ;
    skos:prefLabel "Item I92"@en-AU ;
    dcat:accessURL "https://www.legislation.gov.au/C2004A04997/2024-07-01/2024-07-01/text/1/epub/OEBPS/document_1/document_1.html#_Toc172806592"^^xsd:anyURI .

C2004A04997:93 a C2004A04997:Chapter ;
    rdfs:label "Chapter - C93 Chapter 13 Lac gums resins and other vegetable saps and extracts"@en-AU ;
    dt:isPartOf C2004A04997:61 ;
    rdfs:comment "Chapter 13 Lac gums resins and other vegetable saps and extracts - Abrievated Graph Key: C93"@en-AU ;
    skos:definition "Chapter 13 Lac gums resins and other vegetable saps and extracts"@en-AU ;
    skos:narrower C2004A04997:61 ;
    skos:prefLabel "Chapter C93"@en-AU ;
    dcat:accessURL "https://www.legislation.gov.au/C2004A04997/2024-07-01/2024-07-01/text/1/epub/OEBPS/document_1/document_1.html#_Toc172806593"^^xsd:anyURI .

C2004A04997:94 a C2004A04997:Item ;
    rdfs:label "Item - I94 Note"@en-AU ;
    dt:isPartOf C2004A04997:61 ;
    rdfs:comment "Note - Abrievated Graph Key: I94"@en-AU ;
    skos:definition "Note"@en-AU ;
    skos:narrower C2004A04997:61 ;
    skos:prefLabel "Item I94"@en-AU ;
    dcat:accessURL "https://www.legislation.gov.au/C2004A04997/2024-07-01/2024-07-01/text/1/epub/OEBPS/document_1/document_1.html#_Toc172806594"^^xsd:anyURI .

C2004A04997:95 a C2004A04997:Chapter ;
    rdfs:label "Chapter - C95 Chapter 14 Vegetable plaiting materials vegetable products not elsewhere specified or included"@en-AU ;
    dt:isPartOf C2004A04997:61 ;
    rdfs:comment "Chapter 14 Vegetable plaiting materials vegetable products not elsewhere specified or included - Abrievated Graph Key: C95"@en-AU ;
    skos:definition "Chapter 14 Vegetable plaiting materials vegetable products not elsewhere specified or included"@en-AU ;
    skos:narrower C2004A04997:61 ;
    skos:prefLabel "Chapter C95"@en-AU ;
    dcat:accessURL "https://www.legislation.gov.au/C2004A04997/2024-07-01/2024-07-01/text/1/epub/OEBPS/document_1/document_1.html#_Toc172806595"^^xsd:anyURI .

C2004A04997:96 a C2004A04997:Item ;
    rdfs:label "Item - I96 Notes"@en-AU ;
    dt:isPartOf C2004A04997:61 ;
    rdfs:comment "Notes - Abrievated Graph Key: I96"@en-AU ;
    skos:definition "Notes"@en-AU ;
    skos:narrower C2004A04997:61 ;
    skos:prefLabel "Item I96"@en-AU ;
    dcat:accessURL "https://www.legislation.gov.au/C2004A04997/2024-07-01/2024-07-01/text/1/epub/OEBPS/document_1/document_1.html#_Toc172806596"^^xsd:anyURI .

C2004A04997:97 a C2004A04997:Section ;
    rdfs:label "Section - S97 Section IIIAnimal vegetable or microbial fats and oils and their cleavage products prepared edible fats animal or vegetable waxes"@en-AU ;
    dt:isPartOf C2004A04997:61 ;
    rdfs:comment "Section IIIAnimal vegetable or microbial fats and oils and their cleavage products prepared edible fats animal or vegetable waxes - Abrievated Graph Key: S97"@en-AU ;
    skos:definition "Section IIIAnimal vegetable or microbial fats and oils and their cleavage products prepared edible fats animal or vegetable waxes"@en-AU ;
    skos:narrower C2004A04997:61 ;
    skos:prefLabel "Section S97"@en-AU ;
    dcat:accessURL "https://www.legislation.gov.au/C2004A04997/2024-07-01/2024-07-01/text/1/epub/OEBPS/document_1/document_1.html#_Toc172806597"^^xsd:anyURI .

C2004A04997:98 a C2004A04997:Chapter ;
    rdfs:label "Chapter - C98 Chapter 15 Animal vegetable or microbial fats and oils and their cleavage products prepared edible fats animal or vegetable waxes"@en-AU ;
    dt:isPartOf C2004A04997:61 ;
    rdfs:comment "Chapter 15 Animal vegetable or microbial fats and oils and their cleavage products prepared edible fats animal or vegetable waxes - Abrievated Graph Key: C98"@en-AU ;
    skos:definition "Chapter 15 Animal vegetable or microbial fats and oils and their cleavage products prepared edible fats animal or vegetable waxes"@en-AU ;
    skos:narrower C2004A04997:61 ;
    skos:prefLabel "Chapter C98"@en-AU ;
    dcat:accessURL "https://www.legislation.gov.au/C2004A04997/2024-07-01/2024-07-01/text/1/epub/OEBPS/document_1/document_1.html#_Toc172806598"^^xsd:anyURI .

C2004A04997:99 a C2004A04997:Item ;
    rdfs:label "Item - I99 Notes"@en-AU ;
    dt:isPartOf C2004A04997:61 ;
    rdfs:comment "Notes - Abrievated Graph Key: I99"@en-AU ;
    skos:definition "Notes"@en-AU ;
    skos:narrower C2004A04997:61 ;
    skos:prefLabel "Item I99"@en-AU ;
    dcat:accessURL "https://www.legislation.gov.au/C2004A04997/2024-07-01/2024-07-01/text/1/epub/OEBPS/document_1/document_1.html#_Toc172806599"^^xsd:anyURI .

C2004A04997:Part a legcons:Part,
        owl:Class,
        skos:Concept,
        dcat:Resource ;
    rdfs:label "Part" ;
    skos:prefLabel "Part" .

C2004A04997:281 a C2004A04997:Chapter ;
    rdfs:label "Chapter - C281 Chapter 65 Headgear and parts thereof"@en-AU ;
    dt:hasPart C2004A04997:282 ;
    dt:isPartOf C2004A04997:277 ;
    rdfs:comment "Chapter 65 Headgear and parts thereof - Abrievated Graph Key: C281"@en-AU ;
    skos:broader C2004A04997:282 ;
    skos:definition "Chapter 65 Headgear and parts thereof"@en-AU ;
    skos:narrower C2004A04997:277 ;
    skos:prefLabel "Chapter C281"@en-AU ;
    dcat:accessURL "https://www.legislation.gov.au/C2004A04997/2024-07-01/2024-07-01/text/1/epub/OEBPS/document_4/document_4.html#_Toc171752012"^^xsd:anyURI .

C2004A04997:283 a C2004A04997:Chapter ;
    rdfs:label "Chapter - C283 Chapter 66 Umbrellas sun umbrellas walking sticks seat sticks whips riding crops and parts thereof"@en-AU ;
    dt:hasPart C2004A04997:284 ;
    dt:isPartOf C2004A04997:277 ;
    rdfs:comment "Chapter 66 Umbrellas sun umbrellas walking sticks seat sticks whips riding crops and parts thereof - Abrievated Graph Key: C283"@en-AU ;
    skos:broader C2004A04997:284 ;
    skos:definition "Chapter 66 Umbrellas sun umbrellas walking sticks seat sticks whips riding crops and parts thereof"@en-AU ;
    skos:narrower C2004A04997:277 ;
    skos:prefLabel "Chapter C283"@en-AU ;
    dcat:accessURL "https://www.legislation.gov.au/C2004A04997/2024-07-01/2024-07-01/text/1/epub/OEBPS/document_4/document_4.html#_Toc171752014"^^xsd:anyURI .

C2004A04997:285 a C2004A04997:Chapter ;
    rdfs:label "Chapter - C285 Chapter 67 Prepared feathers and down and articles made of feathers or of down artificial flowers articles of human hair"@en-AU ;
    dt:hasPart C2004A04997:286 ;
    dt:isPartOf C2004A04997:277 ;
    rdfs:comment "Chapter 67 Prepared feathers and down and articles made of feathers or of down artificial flowers articles of human hair - Abrievated Graph Key: C285"@en-AU ;
    skos:broader C2004A04997:286 ;
    skos:definition "Chapter 67 Prepared feathers and down and articles made of feathers or of down artificial flowers articles of human hair"@en-AU ;
    skos:narrower C2004A04997:277 ;
    skos:prefLabel "Chapter C285"@en-AU ;
    dcat:accessURL "https://www.legislation.gov.au/C2004A04997/2024-07-01/2024-07-01/text/1/epub/OEBPS/document_4/document_4.html#_Toc171752016"^^xsd:anyURI .

C2004A04997:288 a C2004A04997:Chapter ;
    rdfs:label "Chapter - C288 Chapter 68 Articles of stone plaster cement asbestos mica or similar materials"@en-AU ;
    dt:hasPart C2004A04997:289 ;
    dt:isPartOf C2004A04997:287 ;
    rdfs:comment "Chapter 68 Articles of stone plaster cement asbestos mica or similar materials - Abrievated Graph Key: C288"@en-AU ;
    skos:broader C2004A04997:289 ;
    skos:definition "Chapter 68 Articles of stone plaster cement asbestos mica or similar materials"@en-AU ;
    skos:narrower C2004A04997:287 ;
    skos:prefLabel "Chapter C288"@en-AU ;
    dcat:accessURL "https://www.legislation.gov.au/C2004A04997/2024-07-01/2024-07-01/text/1/epub/OEBPS/document_4/document_4.html#_Toc171752019"^^xsd:anyURI .

C2004A04997:297 a C2004A04997:Section ;
    rdfs:label "Section - S297 Section XIVNatural or cultured pearls precious or semi precious stones precious metals metals clad with precious metal and articles thereof imitation jewellery coin"@en-AU ;
    dt:hasPart C2004A04997:298 ;
    dt:isPartOf C2004A04997:259 ;
    rdfs:comment "Section XIVNatural or cultured pearls precious or semi precious stones precious metals metals clad with precious metal and articles thereof imitation jewellery coin - Abrievated Graph Key: S297"@en-AU ;
    skos:broader C2004A04997:298 ;
    skos:definition "Section XIVNatural or cultured pearls precious or semi precious stones precious metals metals clad with precious metal and articles thereof imitation jewellery coin"@en-AU ;
    skos:narrower C2004A04997:259 ;
    skos:prefLabel "Section S297"@en-AU ;
    dcat:accessURL "https://www.legislation.gov.au/C2004A04997/2024-07-01/2024-07-01/text/1/epub/OEBPS/document_4/document_4.html#_Toc171752028"^^xsd:anyURI .

C2004A04997:278 a C2004A04997:Chapter ;
    rdfs:label "Chapter - C278 Chapter 64 Footwear gaiters and the like parts of such articles"@en-AU ;
    dt:hasPart C2004A04997:279,
        C2004A04997:280 ;
    dt:isPartOf C2004A04997:277 ;
    rdfs:comment "Chapter 64 Footwear gaiters and the like parts of such articles - Abrievated Graph Key: C278"@en-AU ;
    skos:broader C2004A04997:279,
        C2004A04997:280 ;
    skos:definition "Chapter 64 Footwear gaiters and the like parts of such articles"@en-AU ;
    skos:narrower C2004A04997:277 ;
    skos:prefLabel "Chapter C278"@en-AU ;
    dcat:accessURL "https://www.legislation.gov.au/C2004A04997/2024-07-01/2024-07-01/text/1/epub/OEBPS/document_4/document_4.html#_Toc171752009"^^xsd:anyURI .

C2004A04997:294 a C2004A04997:Chapter ;
    rdfs:label "Chapter - C294 Chapter 70 Glass and glassware"@en-AU ;
    dt:hasPart C2004A04997:295,
        C2004A04997:296 ;
    dt:isPartOf C2004A04997:287 ;
    rdfs:comment "Chapter 70 Glass and glassware - Abrievated Graph Key: C294"@en-AU ;
    skos:broader C2004A04997:295,
        C2004A04997:296 ;
    skos:definition "Chapter 70 Glass and glassware"@en-AU ;
    skos:narrower C2004A04997:287 ;
    skos:prefLabel "Chapter C294"@en-AU ;
    dcat:accessURL "https://www.legislation.gov.au/C2004A04997/2024-07-01/2024-07-01/text/1/epub/OEBPS/document_4/document_4.html#_Toc171752025"^^xsd:anyURI .

C2004A04997:314 a C2004A04997:Chapter ;
    rdfs:label "Chapter - C314 Chapter 73 Articles of iron or steel"@en-AU ;
    dt:hasPart C2004A04997:315,
        C2004A04997:316 ;
    dt:isPartOf C2004A04997:304 ;
    rdfs:comment "Chapter 73 Articles of iron or steel - Abrievated Graph Key: C314"@en-AU ;
    skos:broader C2004A04997:315,
        C2004A04997:316 ;
    skos:definition "Chapter 73 Articles of iron or steel"@en-AU ;
    skos:narrower C2004A04997:304 ;
    skos:prefLabel "Chapter C314"@en-AU ;
    dcat:accessURL "https://www.legislation.gov.au/C2004A04997/2024-07-01/2024-07-01/text/1/epub/OEBPS/document_4/document_4.html#_Toc171752045"^^xsd:anyURI .

C2004A04997:Volume a legcons:Volume,
        owl:Class,
        skos:Concept,
        dcat:Resource ;
    rdfs:label "Volume" ;
    skos:prefLabel "Volume" .

C2004A04997:287 a C2004A04997:Section ;
    rdfs:label "Section - S287 Section XIIIArticles of stone plaster cement asbestos mica or similar materials ceramic products glass and glassware"@en-AU ;
    dt:hasPart C2004A04997:288,
        C2004A04997:290,
        C2004A04997:294 ;
    dt:isPartOf C2004A04997:259 ;
    rdfs:comment "Section XIIIArticles of stone plaster cement asbestos mica or similar materials ceramic products glass and glassware - Abrievated Graph Key: S287"@en-AU ;
    skos:broader C2004A04997:288,
        C2004A04997:290,
        C2004A04997:294 ;
    skos:definition "Section XIIIArticles of stone plaster cement asbestos mica or similar materials ceramic products glass and glassware"@en-AU ;
    skos:narrower C2004A04997:259 ;
    skos:prefLabel "Section S287"@en-AU ;
    dcat:accessURL "https://www.legislation.gov.au/C2004A04997/2024-07-01/2024-07-01/text/1/epub/OEBPS/document_4/document_4.html#_Toc171752018"^^xsd:anyURI .

C2004A04997:290 a C2004A04997:Chapter ;
    rdfs:label "Chapter - C290 Chapter 69 Ceramic products"@en-AU ;
    dt:hasPart C2004A04997:291,
        C2004A04997:292,
        C2004A04997:293 ;
    dt:isPartOf C2004A04997:287 ;
    rdfs:comment "Chapter 69 Ceramic products - Abrievated Graph Key: C290"@en-AU ;
    skos:broader C2004A04997:291,
        C2004A04997:292,
        C2004A04997:293 ;
    skos:definition "Chapter 69 Ceramic products"@en-AU ;
    skos:narrower C2004A04997:287 ;
    skos:prefLabel "Chapter C290"@en-AU ;
    dcat:accessURL "https://www.legislation.gov.au/C2004A04997/2024-07-01/2024-07-01/text/1/epub/OEBPS/document_4/document_4.html#_Toc171752021"^^xsd:anyURI .

C2004A04997:304 a C2004A04997:Section ;
    rdfs:label "Section - S304 Section XVBase metals and articles of base metal"@en-AU ;
    dt:hasPart C2004A04997:305,
        C2004A04997:306,
        C2004A04997:314 ;
    dt:isPartOf C2004A04997:259 ;
    rdfs:comment "Section XVBase metals and articles of base metal - Abrievated Graph Key: S304"@en-AU ;
    skos:broader C2004A04997:305,
        C2004A04997:306,
        C2004A04997:314 ;
    skos:definition "Section XVBase metals and articles of base metal"@en-AU ;
    skos:narrower C2004A04997:259 ;
    skos:prefLabel "Section S304"@en-AU ;
    dcat:accessURL "https://www.legislation.gov.au/C2004A04997/2024-07-01/2024-07-01/text/1/epub/OEBPS/document_4/document_4.html#_Toc171752035"^^xsd:anyURI .

C2004A04997:56 a C2004A04997:Part ;
    rdfs:label "Part - P56 Part 3 Miscellaneous"@en-AU ;
    dt:hasPart C2004A04997:57,
        C2004A04997:58,
        C2004A04997:59 ;
    dt:isPartOf C2004A04997:1 ;
    rdfs:comment "Part 3 Miscellaneous - Abrievated Graph Key: P56"@en-AU ;
    skos:broader C2004A04997:57,
        C2004A04997:58,
        C2004A04997:59 ;
    skos:definition "Part 3 Miscellaneous"@en-AU ;
    skos:narrower C2004A04997:1 ;
    skos:prefLabel "Part P56"@en-AU ;
    dcat:accessURL "https://www.legislation.gov.au/C2004A04997/2024-07-01/2024-07-01/text/1/epub/OEBPS/document_1/document_1.html#_Toc172806556"^^xsd:anyURI .

C2004A04997:1 a C2004A04997:Volume ;
    rdfs:label "Volume - V1 Volume 1"@en-AU ;
    dt:hasPart C2004A04997:2,
        C2004A04997:36,
        C2004A04997:56,
        C2004A04997:60,
        C2004A04997:61 ;
    rdfs:comment "Volume 1 - Abrievated Graph Key: V1"@en-AU ;
    skos:broader C2004A04997:2,
        C2004A04997:36,
        C2004A04997:56,
        C2004A04997:60,
        C2004A04997:61 ;
    skos:definition "Volume 1"@en-AU ;
    skos:prefLabel "Volume V1"@en-AU ;
    dcat:accessURL "https://www.legislation.gov.au/C2004A04997/2024-07-01/2024-07-01/text/1/epub/OEBPS/document_1/document_1.html"^^xsd:anyURI .

C2004A04997:277 a C2004A04997:Section ;
    rdfs:label "Section - S277 Section XIIFootwear headgear umbrellas sun umbrellas walking sticks seat sticks whips riding crops and parts thereof prepared feathers and articles made therewith artificial flowers articles of human hair"@en-AU ;
    dt:hasPart C2004A04997:278,
        C2004A04997:281,
        C2004A04997:283,
        C2004A04997:285 ;
    dt:isPartOf C2004A04997:259 ;
    rdfs:comment "Section XIIFootwear headgear umbrellas sun umbrellas walking sticks seat sticks whips riding crops and parts thereof prepared feathers and articles made therewith artificial flowers articles of human hair - Abrievated Graph Key: S277"@en-AU ;
    skos:broader C2004A04997:278,
        C2004A04997:281,
        C2004A04997:283,
        C2004A04997:285 ;
    skos:definition "Section XIIFootwear headgear umbrellas sun umbrellas walking sticks seat sticks whips riding crops and parts thereof prepared feathers and articles made therewith artificial flowers articles of human hair"@en-AU ;
    skos:narrower C2004A04997:259 ;
    skos:prefLabel "Section S277"@en-AU ;
    dcat:accessURL "https://www.legislation.gov.au/C2004A04997/2024-07-01/2024-07-01/text/1/epub/OEBPS/document_4/document_4.html#_Toc171752008"^^xsd:anyURI .

C2004A04997:408 a C2004A04997:Endnotes ;
    rdfs:label "Endnotes - E408 Endnotes"@en-AU ;
    dt:hasPart C2004A04997:409,
        C2004A04997:410,
        C2004A04997:411,
        C2004A04997:412 ;
    dt:isPartOf C2004A04997:407 ;
    rdfs:comment "Endnotes - Abrievated Graph Key: E408"@en-AU ;
    skos:broader C2004A04997:409,
        C2004A04997:410,
        C2004A04997:411,
        C2004A04997:412 ;
    skos:definition "Endnotes"@en-AU ;
    skos:narrower C2004A04997:407 ;
    skos:prefLabel "Endnotes E408"@en-AU ;
    dcat:accessURL "https://www.legislation.gov.au/C2004A04997/2024-07-01/2024-07-01/text/1/epub/OEBPS/document_7/document_7.html#_Toc171755738"^^xsd:anyURI .

C2004A04997:259 a C2004A04997:Volume ;
    rdfs:label "Volume - V259 Volume 4"@en-AU ;
    dt:hasPart C2004A04997:260,
        C2004A04997:261,
        C2004A04997:277,
        C2004A04997:287,
        C2004A04997:297,
        C2004A04997:304 ;
    rdfs:comment "Volume 4 - Abrievated Graph Key: V259"@en-AU ;
    skos:broader C2004A04997:260,
        C2004A04997:261,
        C2004A04997:277,
        C2004A04997:287,
        C2004A04997:297,
        C2004A04997:304 ;
    skos:definition "Volume 4"@en-AU ;
    skos:prefLabel "Volume V259"@en-AU ;
    dcat:accessURL "https://www.legislation.gov.au/C2004A04997/2024-07-01/2024-07-01/text/1/epub/OEBPS/document_4/document_4.html"^^xsd:anyURI .

C2004A04997:298 a C2004A04997:Chapter ;
    rdfs:label "Chapter - C298 Chapter 71 Natural or cultured pearls precious or semi precious stones precious metals metals clad with precious metal and articles thereof imitation jewellery coin"@en-AU ;
    dt:hasPart C2004A04997:299,
        C2004A04997:300,
        C2004A04997:301,
        C2004A04997:302,
        C2004A04997:303 ;
    dt:isPartOf C2004A04997:297 ;
    rdfs:comment "Chapter 71 Natural or cultured pearls precious or semi precious stones precious metals metals clad with precious metal and articles thereof imitation jewellery coin - Abrievated Graph Key: C298"@en-AU ;
    skos:broader C2004A04997:299,
        C2004A04997:300,
        C2004A04997:301,
        C2004A04997:302,
        C2004A04997:303 ;
    skos:definition "Chapter 71 Natural or cultured pearls precious or semi precious stones precious metals metals clad with precious metal and articles thereof imitation jewellery coin"@en-AU ;
    skos:narrower C2004A04997:297 ;
    skos:prefLabel "Chapter C298"@en-AU ;
    dcat:accessURL "https://www.legislation.gov.au/C2004A04997/2024-07-01/2024-07-01/text/1/epub/OEBPS/document_4/document_4.html#_Toc171752029"^^xsd:anyURI .

C2004A04997:306 a C2004A04997:Chapter ;
    rdfs:label "Chapter - C306 Chapter 72 Iron and steel"@en-AU ;
    dt:hasPart C2004A04997:307,
        C2004A04997:308,
        C2004A04997:309,
        C2004A04997:310,
        C2004A04997:311,
        C2004A04997:312,
        C2004A04997:313 ;
    dt:isPartOf C2004A04997:304 ;
    rdfs:comment "Chapter 72 Iron and steel - Abrievated Graph Key: C306"@en-AU ;
    skos:broader C2004A04997:307,
        C2004A04997:308,
        C2004A04997:309,
        C2004A04997:310,
        C2004A04997:311,
        C2004A04997:312,
        C2004A04997:313 ;
    skos:definition "Chapter 72 Iron and steel"@en-AU ;
    skos:narrower C2004A04997:304 ;
    skos:prefLabel "Chapter C306"@en-AU ;
    dcat:accessURL "https://www.legislation.gov.au/C2004A04997/2024-07-01/2024-07-01/text/1/epub/OEBPS/document_4/document_4.html#_Toc171752037"^^xsd:anyURI .

C2004A04997:Section a legcons:Section,
        owl:Class,
        skos:Concept,
        dcat:Resource ;
    rdfs:label "Section" ;
    skos:prefLabel "Section" .

C2004A04997:Schedule a legcons:Schedule,
        owl:Class,
        skos:Concept,
        dcat:Resource ;
    rdfs:label "Schedule" ;
    skos:prefLabel "Schedule" .

C2004A04997:62 a C2004A04997:Section ;
    rdfs:label "Section - S62 Section ILive animals animal products"@en-AU ;
    dt:hasPart C2004A04997:63,
        C2004A04997:64,
        C2004A04997:65,
        C2004A04997:66,
        C2004A04997:67,
        C2004A04997:68,
        C2004A04997:69,
        C2004A04997:70,
        C2004A04997:71,
        C2004A04997:72,
        C2004A04997:73,
        C2004A04997:74 ;
    dt:isPartOf C2004A04997:61 ;
    rdfs:comment "Section ILive animals animal products - Abrievated Graph Key: S62"@en-AU ;
    skos:broader C2004A04997:63,
        C2004A04997:64,
        C2004A04997:65,
        C2004A04997:66,
        C2004A04997:67,
        C2004A04997:68,
        C2004A04997:69,
        C2004A04997:70,
        C2004A04997:71,
        C2004A04997:72,
        C2004A04997:73,
        C2004A04997:74 ;
    skos:definition "Section ILive animals animal products"@en-AU ;
    skos:narrower C2004A04997:61 ;
    skos:prefLabel "Section S62"@en-AU ;
    dcat:accessURL "https://www.legislation.gov.au/C2004A04997/2024-07-01/2024-07-01/text/1/epub/OEBPS/document_1/document_1.html#_Toc172806562"^^xsd:anyURI .

C2004A04997:261 a C2004A04997:Section ;
    rdfs:label "Section - S261 Section XITextiles and textile articles"@en-AU ;
    dt:hasPart C2004A04997:262,
        C2004A04997:263,
        C2004A04997:264,
        C2004A04997:265,
        C2004A04997:266,
        C2004A04997:267,
        C2004A04997:268,
        C2004A04997:269,
        C2004A04997:270,
        C2004A04997:271,
        C2004A04997:272,
        C2004A04997:273,
        C2004A04997:274,
        C2004A04997:275,
        C2004A04997:276 ;
    dt:isPartOf C2004A04997:259 ;
    rdfs:comment "Section XITextiles and textile articles - Abrievated Graph Key: S261"@en-AU ;
    skos:broader C2004A04997:262,
        C2004A04997:263,
        C2004A04997:264,
        C2004A04997:265,
        C2004A04997:266,
        C2004A04997:267,
        C2004A04997:268,
        C2004A04997:269,
        C2004A04997:270,
        C2004A04997:271,
        C2004A04997:272,
        C2004A04997:273,
        C2004A04997:274,
        C2004A04997:275,
        C2004A04997:276 ;
    skos:definition "Section XITextiles and textile articles"@en-AU ;
    skos:narrower C2004A04997:259 ;
    skos:prefLabel "Section S261"@en-AU ;
    dcat:accessURL "https://www.legislation.gov.au/C2004A04997/2024-07-01/2024-07-01/text/1/epub/OEBPS/document_4/document_4.html#_Toc171751992"^^xsd:anyURI .

C2004A04997:388 a C2004A04997:Volume ;
    rdfs:label "Volume - V388 Volume 6"@en-AU ;
    dt:hasPart C2004A04997:389,
        C2004A04997:390,
        C2004A04997:391,
        C2004A04997:392,
        C2004A04997:393,
        C2004A04997:394,
        C2004A04997:395,
        C2004A04997:396,
        C2004A04997:397,
        C2004A04997:398,
        C2004A04997:399,
        C2004A04997:400,
        C2004A04997:401,
        C2004A04997:402,
        C2004A04997:403,
        C2004A04997:404,
        C2004A04997:405,
        C2004A04997:406 ;
    rdfs:comment "Volume 6 - Abrievated Graph Key: V388"@en-AU ;
    skos:broader C2004A04997:389,
        C2004A04997:390,
        C2004A04997:391,
        C2004A04997:392,
        C2004A04997:393,
        C2004A04997:394,
        C2004A04997:395,
        C2004A04997:396,
        C2004A04997:397,
        C2004A04997:398,
        C2004A04997:399,
        C2004A04997:400,
        C2004A04997:401,
        C2004A04997:402,
        C2004A04997:403,
        C2004A04997:404,
        C2004A04997:405,
        C2004A04997:406 ;
    skos:definition "Volume 6"@en-AU ;
    skos:prefLabel "Volume V388"@en-AU ;
    dcat:accessURL "https://www.legislation.gov.au/C2004A04997/2024-07-01/2024-07-01/text/1/epub/OEBPS/document_6/document_6.html"^^xsd:anyURI .

C2004A04997:36 a C2004A04997:Part ;
    rdfs:label "Part - P36 Part 2 Duties of Customs"@en-AU ;
    dt:hasPart C2004A04997:37,
        C2004A04997:38,
        C2004A04997:39,
        C2004A04997:40,
        C2004A04997:41,
        C2004A04997:42,
        C2004A04997:43,
        C2004A04997:44,
        C2004A04997:45,
        C2004A04997:46,
        C2004A04997:47,
        C2004A04997:48,
        C2004A04997:49,
        C2004A04997:50,
        C2004A04997:51,
        C2004A04997:52,
        C2004A04997:53,
        C2004A04997:54,
        C2004A04997:55 ;
    dt:isPartOf C2004A04997:1 ;
    rdfs:comment "Part 2 Duties of Customs - Abrievated Graph Key: P36"@en-AU ;
    skos:broader C2004A04997:37,
        C2004A04997:38,
        C2004A04997:39,
        C2004A04997:40,
        C2004A04997:41,
        C2004A04997:42,
        C2004A04997:43,
        C2004A04997:44,
        C2004A04997:45,
        C2004A04997:46,
        C2004A04997:47,
        C2004A04997:48,
        C2004A04997:49,
        C2004A04997:50,
        C2004A04997:51,
        C2004A04997:52,
        C2004A04997:53,
        C2004A04997:54,
        C2004A04997:55 ;
    skos:definition "Part 2 Duties of Customs"@en-AU ;
    skos:narrower C2004A04997:1 ;
    skos:prefLabel "Part P36"@en-AU ;
    dcat:accessURL "https://www.legislation.gov.au/C2004A04997/2024-07-01/2024-07-01/text/1/epub/OEBPS/document_1/document_1.html#_Toc172806536"^^xsd:anyURI .

C2004A04997:61 a C2004A04997:Schedule ;
    rdfs:label "Schedule - S61 Schedule 3 Classification of goods and general and special rates of duty"@en-AU ;
    dt:hasPart C2004A04997:100,
        C2004A04997:101,
        C2004A04997:62,
        C2004A04997:75,
        C2004A04997:76,
        C2004A04997:77,
        C2004A04997:78,
        C2004A04997:79,
        C2004A04997:80,
        C2004A04997:81,
        C2004A04997:82,
        C2004A04997:83,
        C2004A04997:84,
        C2004A04997:85,
        C2004A04997:86,
        C2004A04997:87,
        C2004A04997:88,
        C2004A04997:89,
        C2004A04997:90,
        C2004A04997:91,
        C2004A04997:92,
        C2004A04997:93,
        C2004A04997:94,
        C2004A04997:95,
        C2004A04997:96,
        C2004A04997:97,
        C2004A04997:98,
        C2004A04997:99 ;
    dt:isPartOf C2004A04997:1 ;
    rdfs:comment "Schedule 3 Classification of goods and general and special rates of duty - Abrievated Graph Key: S61"@en-AU ;
    skos:broader C2004A04997:100,
        C2004A04997:101,
        C2004A04997:62,
        C2004A04997:75,
        C2004A04997:76,
        C2004A04997:77,
        C2004A04997:78,
        C2004A04997:79,
        C2004A04997:80,
        C2004A04997:81,
        C2004A04997:82,
        C2004A04997:83,
        C2004A04997:84,
        C2004A04997:85,
        C2004A04997:86,
        C2004A04997:87,
        C2004A04997:88,
        C2004A04997:89,
        C2004A04997:90,
        C2004A04997:91,
        C2004A04997:92,
        C2004A04997:93,
        C2004A04997:94,
        C2004A04997:95,
        C2004A04997:96,
        C2004A04997:97,
        C2004A04997:98,
        C2004A04997:99 ;
    skos:definition "Schedule 3 Classification of goods and general and special rates of duty"@en-AU ;
    skos:narrower C2004A04997:1 ;
    skos:prefLabel "Schedule S61"@en-AU ;
    dcat:accessURL "https://www.legislation.gov.au/C2004A04997/2024-07-01/2024-07-01/text/1/epub/OEBPS/document_1/document_1.html#_Toc172806561"^^xsd:anyURI .

C2004A04997:2 a C2004A04997:Part ;
    rdfs:label "Part - P2 Part 1 Preliminary"@en-AU ;
    dt:hasPart C2004A04997:10,
        C2004A04997:11,
        C2004A04997:12,
        C2004A04997:13,
        C2004A04997:14,
        C2004A04997:15,
        C2004A04997:16,
        C2004A04997:17,
        C2004A04997:18,
        C2004A04997:19,
        C2004A04997:20,
        C2004A04997:21,
        C2004A04997:22,
        C2004A04997:23,
        C2004A04997:24,
        C2004A04997:25,
        C2004A04997:26,
        C2004A04997:27,
        C2004A04997:28,
        C2004A04997:29,
        C2004A04997:3,
        C2004A04997:30,
        C2004A04997:31,
        C2004A04997:32,
        C2004A04997:33,
        C2004A04997:34,
        C2004A04997:35,
        C2004A04997:4,
        C2004A04997:5,
        C2004A04997:6,
        C2004A04997:7,
        C2004A04997:8,
        C2004A04997:9 ;
    dt:isPartOf C2004A04997:1 ;
    rdfs:comment "Part 1 Preliminary - Abrievated Graph Key: P2"@en-AU ;
    skos:broader C2004A04997:10,
        C2004A04997:11,
        C2004A04997:12,
        C2004A04997:13,
        C2004A04997:14,
        C2004A04997:15,
        C2004A04997:16,
        C2004A04997:17,
        C2004A04997:18,
        C2004A04997:19,
        C2004A04997:20,
        C2004A04997:21,
        C2004A04997:22,
        C2004A04997:23,
        C2004A04997:24,
        C2004A04997:25,
        C2004A04997:26,
        C2004A04997:27,
        C2004A04997:28,
        C2004A04997:29,
        C2004A04997:3,
        C2004A04997:30,
        C2004A04997:31,
        C2004A04997:32,
        C2004A04997:33,
        C2004A04997:34,
        C2004A04997:35,
        C2004A04997:4,
        C2004A04997:5,
        C2004A04997:6,
        C2004A04997:7,
        C2004A04997:8,
        C2004A04997:9 ;
    skos:definition "Part 1 Preliminary"@en-AU ;
    skos:narrower C2004A04997:1 ;
    skos:prefLabel "Part P2"@en-AU ;
    dcat:accessURL "https://www.legislation.gov.au/C2004A04997/2024-07-01/2024-07-01/text/1/epub/OEBPS/document_1/document_1.html#_Toc172806502"^^xsd:anyURI .

C2004A04997:Chapter a legcons:Chapter,
        owl:Class,
        skos:Concept,
        dcat:Resource ;
    rdfs:label "Chapter" ;
    skos:prefLabel "Chapter" .

C2004A04997:198 a C2004A04997:Schedule ;
    rdfs:label "Schedule - S198 Schedule 3 Classification of goods and general and special rates of duty"@en-AU ;
    dt:hasPart C2004A04997:199,
        C2004A04997:200,
        C2004A04997:201,
        C2004A04997:202,
        C2004A04997:203,
        C2004A04997:204,
        C2004A04997:205,
        C2004A04997:206,
        C2004A04997:207,
        C2004A04997:208,
        C2004A04997:209,
        C2004A04997:210,
        C2004A04997:211,
        C2004A04997:212,
        C2004A04997:213,
        C2004A04997:214,
        C2004A04997:215,
        C2004A04997:216,
        C2004A04997:217,
        C2004A04997:218,
        C2004A04997:219,
        C2004A04997:220,
        C2004A04997:221,
        C2004A04997:222,
        C2004A04997:223,
        C2004A04997:224,
        C2004A04997:225,
        C2004A04997:226,
        C2004A04997:227,
        C2004A04997:228,
        C2004A04997:229,
        C2004A04997:230,
        C2004A04997:231,
        C2004A04997:232,
        C2004A04997:233,
        C2004A04997:234,
        C2004A04997:235,
        C2004A04997:236,
        C2004A04997:237,
        C2004A04997:238,
        C2004A04997:239,
        C2004A04997:240,
        C2004A04997:241,
        C2004A04997:242,
        C2004A04997:243,
        C2004A04997:244,
        C2004A04997:245,
        C2004A04997:246,
        C2004A04997:247,
        C2004A04997:248,
        C2004A04997:249,
        C2004A04997:250,
        C2004A04997:251,
        C2004A04997:252,
        C2004A04997:253,
        C2004A04997:254,
        C2004A04997:255,
        C2004A04997:256,
        C2004A04997:257,
        C2004A04997:258 ;
    dt:isPartOf C2004A04997:197 ;
    rdfs:comment "Schedule 3 Classification of goods and general and special rates of duty - Abrievated Graph Key: S198"@en-AU ;
    skos:broader C2004A04997:199,
        C2004A04997:200,
        C2004A04997:201,
        C2004A04997:202,
        C2004A04997:203,
        C2004A04997:204,
        C2004A04997:205,
        C2004A04997:206,
        C2004A04997:207,
        C2004A04997:208,
        C2004A04997:209,
        C2004A04997:210,
        C2004A04997:211,
        C2004A04997:212,
        C2004A04997:213,
        C2004A04997:214,
        C2004A04997:215,
        C2004A04997:216,
        C2004A04997:217,
        C2004A04997:218,
        C2004A04997:219,
        C2004A04997:220,
        C2004A04997:221,
        C2004A04997:222,
        C2004A04997:223,
        C2004A04997:224,
        C2004A04997:225,
        C2004A04997:226,
        C2004A04997:227,
        C2004A04997:228,
        C2004A04997:229,
        C2004A04997:230,
        C2004A04997:231,
        C2004A04997:232,
        C2004A04997:233,
        C2004A04997:234,
        C2004A04997:235,
        C2004A04997:236,
        C2004A04997:237,
        C2004A04997:238,
        C2004A04997:239,
        C2004A04997:240,
        C2004A04997:241,
        C2004A04997:242,
        C2004A04997:243,
        C2004A04997:244,
        C2004A04997:245,
        C2004A04997:246,
        C2004A04997:247,
        C2004A04997:248,
        C2004A04997:249,
        C2004A04997:250,
        C2004A04997:251,
        C2004A04997:252,
        C2004A04997:253,
        C2004A04997:254,
        C2004A04997:255,
        C2004A04997:256,
        C2004A04997:257,
        C2004A04997:258 ;
    skos:definition "Schedule 3 Classification of goods and general and special rates of duty"@en-AU ;
    skos:narrower C2004A04997:197 ;
    skos:prefLabel "Schedule S198"@en-AU ;
    dcat:accessURL "https://www.legislation.gov.au/C2004A04997/2024-07-01/2024-07-01/text/1/epub/OEBPS/document_3/document_3.html#_Toc171751528"^^xsd:anyURI .

C2004A04997:318 a C2004A04997:Schedule ;
    rdfs:label "Schedule - S318 Schedule 3 Classification of goods and general and special rates of duty"@en-AU ;
    dt:hasPart C2004A04997:319,
        C2004A04997:320,
        C2004A04997:321,
        C2004A04997:322,
        C2004A04997:323,
        C2004A04997:324,
        C2004A04997:325,
        C2004A04997:326,
        C2004A04997:327,
        C2004A04997:328,
        C2004A04997:329,
        C2004A04997:330,
        C2004A04997:331,
        C2004A04997:332,
        C2004A04997:333,
        C2004A04997:334,
        C2004A04997:335,
        C2004A04997:336,
        C2004A04997:337,
        C2004A04997:338,
        C2004A04997:339,
        C2004A04997:340,
        C2004A04997:341,
        C2004A04997:342,
        C2004A04997:343,
        C2004A04997:344,
        C2004A04997:345,
        C2004A04997:346,
        C2004A04997:347,
        C2004A04997:348,
        C2004A04997:349,
        C2004A04997:350,
        C2004A04997:351,
        C2004A04997:352,
        C2004A04997:353,
        C2004A04997:354,
        C2004A04997:355,
        C2004A04997:356,
        C2004A04997:357,
        C2004A04997:358,
        C2004A04997:359,
        C2004A04997:360,
        C2004A04997:361,
        C2004A04997:362,
        C2004A04997:363,
        C2004A04997:364,
        C2004A04997:365,
        C2004A04997:366,
        C2004A04997:367,
        C2004A04997:368,
        C2004A04997:369,
        C2004A04997:370,
        C2004A04997:371,
        C2004A04997:372,
        C2004A04997:373,
        C2004A04997:374,
        C2004A04997:375,
        C2004A04997:376,
        C2004A04997:377,
        C2004A04997:378,
        C2004A04997:379,
        C2004A04997:380,
        C2004A04997:381,
        C2004A04997:382,
        C2004A04997:383,
        C2004A04997:384,
        C2004A04997:385,
        C2004A04997:386,
        C2004A04997:387 ;
    dt:isPartOf C2004A04997:317 ;
    rdfs:comment "Schedule 3 Classification of goods and general and special rates of duty - Abrievated Graph Key: S318"@en-AU ;
    skos:broader C2004A04997:319,
        C2004A04997:320,
        C2004A04997:321,
        C2004A04997:322,
        C2004A04997:323,
        C2004A04997:324,
        C2004A04997:325,
        C2004A04997:326,
        C2004A04997:327,
        C2004A04997:328,
        C2004A04997:329,
        C2004A04997:330,
        C2004A04997:331,
        C2004A04997:332,
        C2004A04997:333,
        C2004A04997:334,
        C2004A04997:335,
        C2004A04997:336,
        C2004A04997:337,
        C2004A04997:338,
        C2004A04997:339,
        C2004A04997:340,
        C2004A04997:341,
        C2004A04997:342,
        C2004A04997:343,
        C2004A04997:344,
        C2004A04997:345,
        C2004A04997:346,
        C2004A04997:347,
        C2004A04997:348,
        C2004A04997:349,
        C2004A04997:350,
        C2004A04997:351,
        C2004A04997:352,
        C2004A04997:353,
        C2004A04997:354,
        C2004A04997:355,
        C2004A04997:356,
        C2004A04997:357,
        C2004A04997:358,
        C2004A04997:359,
        C2004A04997:360,
        C2004A04997:361,
        C2004A04997:362,
        C2004A04997:363,
        C2004A04997:364,
        C2004A04997:365,
        C2004A04997:366,
        C2004A04997:367,
        C2004A04997:368,
        C2004A04997:369,
        C2004A04997:370,
        C2004A04997:371,
        C2004A04997:372,
        C2004A04997:373,
        C2004A04997:374,
        C2004A04997:375,
        C2004A04997:376,
        C2004A04997:377,
        C2004A04997:378,
        C2004A04997:379,
        C2004A04997:380,
        C2004A04997:381,
        C2004A04997:382,
        C2004A04997:383,
        C2004A04997:384,
        C2004A04997:385,
        C2004A04997:386,
        C2004A04997:387 ;
    skos:definition "Schedule 3 Classification of goods and general and special rates of duty"@en-AU ;
    skos:narrower C2004A04997:317 ;
    skos:prefLabel "Schedule S318"@en-AU ;
    dcat:accessURL "https://www.legislation.gov.au/C2004A04997/2024-07-01/2024-07-01/text/1/epub/OEBPS/document_5/document_5.html#_Toc171753160"^^xsd:anyURI .

C2004A04997:103 a C2004A04997:Schedule ;
    rdfs:label "Schedule - S103 Schedule 3 Classification of goods and general and special rates of duty"@en-AU ;
    dt:hasPart C2004A04997:104,
        C2004A04997:105,
        C2004A04997:106,
        C2004A04997:107,
        C2004A04997:108,
        C2004A04997:109,
        C2004A04997:110,
        C2004A04997:111,
        C2004A04997:112,
        C2004A04997:113,
        C2004A04997:114,
        C2004A04997:115,
        C2004A04997:116,
        C2004A04997:117,
        C2004A04997:118,
        C2004A04997:119,
        C2004A04997:120,
        C2004A04997:121,
        C2004A04997:122,
        C2004A04997:123,
        C2004A04997:124,
        C2004A04997:125,
        C2004A04997:126,
        C2004A04997:127,
        C2004A04997:128,
        C2004A04997:129,
        C2004A04997:130,
        C2004A04997:131,
        C2004A04997:132,
        C2004A04997:133,
        C2004A04997:134,
        C2004A04997:135,
        C2004A04997:136,
        C2004A04997:137,
        C2004A04997:138,
        C2004A04997:139,
        C2004A04997:140,
        C2004A04997:141,
        C2004A04997:142,
        C2004A04997:143,
        C2004A04997:144,
        C2004A04997:145,
        C2004A04997:146,
        C2004A04997:147,
        C2004A04997:148,
        C2004A04997:149,
        C2004A04997:150,
        C2004A04997:151,
        C2004A04997:152,
        C2004A04997:153,
        C2004A04997:154,
        C2004A04997:155,
        C2004A04997:156,
        C2004A04997:157,
        C2004A04997:158,
        C2004A04997:159,
        C2004A04997:160,
        C2004A04997:161,
        C2004A04997:162,
        C2004A04997:163,
        C2004A04997:164,
        C2004A04997:165,
        C2004A04997:166,
        C2004A04997:167,
        C2004A04997:168,
        C2004A04997:169,
        C2004A04997:170,
        C2004A04997:171,
        C2004A04997:172,
        C2004A04997:173,
        C2004A04997:174,
        C2004A04997:175,
        C2004A04997:176,
        C2004A04997:177,
        C2004A04997:178,
        C2004A04997:179,
        C2004A04997:180,
        C2004A04997:181,
        C2004A04997:182,
        C2004A04997:183,
        C2004A04997:184,
        C2004A04997:185,
        C2004A04997:186,
        C2004A04997:187,
        C2004A04997:188,
        C2004A04997:189,
        C2004A04997:190,
        C2004A04997:191,
        C2004A04997:192,
        C2004A04997:193,
        C2004A04997:194,
        C2004A04997:195,
        C2004A04997:196 ;
    dt:isPartOf C2004A04997:102 ;
    rdfs:comment "Schedule 3 Classification of goods and general and special rates of duty - Abrievated Graph Key: S103"@en-AU ;
    skos:broader C2004A04997:104,
        C2004A04997:105,
        C2004A04997:106,
        C2004A04997:107,
        C2004A04997:108,
        C2004A04997:109,
        C2004A04997:110,
        C2004A04997:111,
        C2004A04997:112,
        C2004A04997:113,
        C2004A04997:114,
        C2004A04997:115,
        C2004A04997:116,
        C2004A04997:117,
        C2004A04997:118,
        C2004A04997:119,
        C2004A04997:120,
        C2004A04997:121,
        C2004A04997:122,
        C2004A04997:123,
        C2004A04997:124,
        C2004A04997:125,
        C2004A04997:126,
        C2004A04997:127,
        C2004A04997:128,
        C2004A04997:129,
        C2004A04997:130,
        C2004A04997:131,
        C2004A04997:132,
        C2004A04997:133,
        C2004A04997:134,
        C2004A04997:135,
        C2004A04997:136,
        C2004A04997:137,
        C2004A04997:138,
        C2004A04997:139,
        C2004A04997:140,
        C2004A04997:141,
        C2004A04997:142,
        C2004A04997:143,
        C2004A04997:144,
        C2004A04997:145,
        C2004A04997:146,
        C2004A04997:147,
        C2004A04997:148,
        C2004A04997:149,
        C2004A04997:150,
        C2004A04997:151,
        C2004A04997:152,
        C2004A04997:153,
        C2004A04997:154,
        C2004A04997:155,
        C2004A04997:156,
        C2004A04997:157,
        C2004A04997:158,
        C2004A04997:159,
        C2004A04997:160,
        C2004A04997:161,
        C2004A04997:162,
        C2004A04997:163,
        C2004A04997:164,
        C2004A04997:165,
        C2004A04997:166,
        C2004A04997:167,
        C2004A04997:168,
        C2004A04997:169,
        C2004A04997:170,
        C2004A04997:171,
        C2004A04997:172,
        C2004A04997:173,
        C2004A04997:174,
        C2004A04997:175,
        C2004A04997:176,
        C2004A04997:177,
        C2004A04997:178,
        C2004A04997:179,
        C2004A04997:180,
        C2004A04997:181,
        C2004A04997:182,
        C2004A04997:183,
        C2004A04997:184,
        C2004A04997:185,
        C2004A04997:186,
        C2004A04997:187,
        C2004A04997:188,
        C2004A04997:189,
        C2004A04997:190,
        C2004A04997:191,
        C2004A04997:192,
        C2004A04997:193,
        C2004A04997:194,
        C2004A04997:195,
        C2004A04997:196 ;
    skos:definition "Schedule 3 Classification of goods and general and special rates of duty"@en-AU ;
    skos:narrower C2004A04997:102 ;
    skos:prefLabel "Schedule S103"@en-AU ;
    dcat:accessURL "https://www.legislation.gov.au/C2004A04997/2024-07-01/2024-07-01/text/1/epub/OEBPS/document_2/document_2.html#_Toc171750929"^^xsd:anyURI .

C2004A04997:Item a legcons:Item,
        owl:Class,
        skos:Concept,
        dcat:Resource ;
    rdfs:label "Item" ;
    skos:prefLabel "Item" .

