@prefix C2004A04997: <http://example.org/au/leg/dataset/C2004A04997/> .
@prefix dcat: <http://www.w3.org/ns/dcat#> .
@prefix dct: <http://purl.org/dc/terms/> .
@prefix legcons: <http://example.org/au/leg/concepts/> .
@prefix owl: <http://www.w3.org/2002/07/owl#> .
@prefix rdfs: <http://www.w3.org/2000/01/rdf-schema#> .
@prefix schema: <https://schema.org/> .
@prefix skos: <http://www.w3.org/2004/02/skos/core#> .
@prefix xsd: <http://www.w3.org/2001/XMLSchema#> .

C2004A04997:10 a legcons:Item,
        C2004A04997:Item,
        owl:Class,
        dcat:Resource ;
    rdfs:label "Item - I10 7  Rules for classifying goods in Schedule 3"@en-AU ;
    dct:isPartOf C2004A04997:2 ;
    rdfs:comment "7  Rules for classifying goods in Schedule 3 - Abrievated Graph Key: I10"@en-AU ;
    rdfs:subClassOf C2004A04997: ;
    skos:definition "7  Rules for classifying goods in Schedule 3"@en-AU ;
    skos:narrower C2004A04997:2 ;
    skos:prefLabel "Item I10"@en-AU ;
    dcat:accessURL <https://www.legislation.gov.au/C2004A04997/2024-07-01/2024-07-01/text/1/epub/OEBPS/document_1/document_1.html#_Toc172806510> ;
    dcat:landingPage "https://www.legislation.gov.au/C2004A04997/2024-07-01/2024-07-01/text/1/epub/OEBPS/document_1/document_1.html#_Toc172806510"^^xsd:anyURI ;
    dcat:theme legcons:Item .

C2004A04997:100 a legcons:Item,
        C2004A04997:Item,
        owl:Class,
        dcat:Resource ;
    rdfs:label "Item - I100 Subheading Notes"@en-AU ;
    dct:isPartOf C2004A04997:61 ;
    rdfs:comment "Subheading Notes - Abrievated Graph Key: I100"@en-AU ;
    rdfs:subClassOf C2004A04997: ;
    skos:definition "Subheading Notes"@en-AU ;
    skos:narrower C2004A04997:61 ;
    skos:prefLabel "Item I100"@en-AU ;
    dcat:accessURL <https://www.legislation.gov.au/C2004A04997/2024-07-01/2024-07-01/text/1/epub/OEBPS/document_1/document_1.html#_Toc172806600> ;
    dcat:landingPage "https://www.legislation.gov.au/C2004A04997/2024-07-01/2024-07-01/text/1/epub/OEBPS/document_1/document_1.html#_Toc172806600"^^xsd:anyURI ;
    dcat:theme legcons:Item .

C2004A04997:101 a legcons:Item,
        C2004A04997:Item,
        owl:Class,
        dcat:Resource ;
    rdfs:label "Item - I101 Additional Note"@en-AU ;
    dct:isPartOf C2004A04997:61 ;
    rdfs:comment "Additional Note - Abrievated Graph Key: I101"@en-AU ;
    rdfs:subClassOf C2004A04997: ;
    skos:definition "Additional Note"@en-AU ;
    skos:narrower C2004A04997:61 ;
    skos:prefLabel "Item I101"@en-AU ;
    dcat:accessURL <https://www.legislation.gov.au/C2004A04997/2024-07-01/2024-07-01/text/1/epub/OEBPS/document_1/document_1.html#_Toc172806601> ;
    dcat:landingPage "https://www.legislation.gov.au/C2004A04997/2024-07-01/2024-07-01/text/1/epub/OEBPS/document_1/document_1.html#_Toc172806601"^^xsd:anyURI ;
    dcat:theme legcons:Item .

C2004A04997:102 a legcons:Volume,
        C2004A04997:Volume,
        owl:Class,
        dcat:Resource ;
    rdfs:label "Volume - V102 Volume 2"@en-AU ;
    dct:hasPart C2004A04997:103 ;
    rdfs:comment "Volume 2 - Abrievated Graph Key: V102"@en-AU ;
    rdfs:subClassOf C2004A04997: ;
    skos:broader C2004A04997:103 ;
    skos:definition "Volume 2"@en-AU ;
    skos:prefLabel "Volume V102"@en-AU ;
    dcat:accessURL <https://www.legislation.gov.au/C2004A04997/2024-07-01/2024-07-01/text/1/epub/OEBPS/document_2/document_2.html> ;
    dcat:landingPage "https://www.legislation.gov.au/C2004A04997/2024-07-01/2024-07-01/text/1/epub/OEBPS/document_2/document_2.html"^^xsd:anyURI ;
    dcat:theme legcons:Volume .

C2004A04997:104 a legcons:Section,
        C2004A04997:Section,
        owl:Class,
        dcat:Resource ;
    rdfs:label "Section - S104 Section IVPrepared foodstuffs beverages spirits and vinegar tobacco and manufactured tobacco substitutes products whether or not containing nicotine intended for inhalation without combustion other nicotine containing products intended for the intake of nicotine into the human body"@en-AU ;
    dct:isPartOf C2004A04997:103 ;
    rdfs:comment "Section IVPrepared foodstuffs beverages spirits and vinegar tobacco and manufactured tobacco substitutes products whether or not containing nicotine intended for inhalation without combustion other nicotine containing products intended for the intake of nicotine into the human body - Abrievated Graph Key: S104"@en-AU ;
    rdfs:subClassOf C2004A04997: ;
    skos:definition "Section IVPrepared foodstuffs beverages spirits and vinegar tobacco and manufactured tobacco substitutes products whether or not containing nicotine intended for inhalation without combustion other nicotine containing products intended for the intake of nicotine into the human body"@en-AU ;
    skos:narrower C2004A04997:103 ;
    skos:prefLabel "Section S104"@en-AU ;
    dcat:accessURL <https://www.legislation.gov.au/C2004A04997/2024-07-01/2024-07-01/text/1/epub/OEBPS/document_2/document_2.html#_Toc171750930> ;
    dcat:landingPage "https://www.legislation.gov.au/C2004A04997/2024-07-01/2024-07-01/text/1/epub/OEBPS/document_2/document_2.html#_Toc171750930"^^xsd:anyURI ;
    dcat:theme legcons:Section .

C2004A04997:105 a legcons:Item,
        C2004A04997:Item,
        owl:Class,
        dcat:Resource ;
    rdfs:label "Item - I105 Note"@en-AU ;
    dct:isPartOf C2004A04997:103 ;
    rdfs:comment "Note - Abrievated Graph Key: I105"@en-AU ;
    rdfs:subClassOf C2004A04997: ;
    skos:definition "Note"@en-AU ;
    skos:narrower C2004A04997:103 ;
    skos:prefLabel "Item I105"@en-AU ;
    dcat:accessURL <https://www.legislation.gov.au/C2004A04997/2024-07-01/2024-07-01/text/1/epub/OEBPS/document_2/document_2.html#_Toc171750931> ;
    dcat:landingPage "https://www.legislation.gov.au/C2004A04997/2024-07-01/2024-07-01/text/1/epub/OEBPS/document_2/document_2.html#_Toc171750931"^^xsd:anyURI ;
    dcat:theme legcons:Item .

C2004A04997:106 a legcons:Item,
        C2004A04997:Item,
        owl:Class,
        dcat:Resource ;
    rdfs:label "Item - I106 Additional Note"@en-AU ;
    dct:isPartOf C2004A04997:103 ;
    rdfs:comment "Additional Note - Abrievated Graph Key: I106"@en-AU ;
    rdfs:subClassOf C2004A04997: ;
    skos:definition "Additional Note"@en-AU ;
    skos:narrower C2004A04997:103 ;
    skos:prefLabel "Item I106"@en-AU ;
    dcat:accessURL <https://www.legislation.gov.au/C2004A04997/2024-07-01/2024-07-01/text/1/epub/OEBPS/document_2/document_2.html#_Toc171750932> ;
    dcat:landingPage "https://www.legislation.gov.au/C2004A04997/2024-07-01/2024-07-01/text/1/epub/OEBPS/document_2/document_2.html#_Toc171750932"^^xsd:anyURI ;
    dcat:theme legcons:Item .

C2004A04997:107 a legcons:Chapter,
        C2004A04997:Chapter,
        owl:Class,
        dcat:Resource ;
    rdfs:label "Chapter - C107 Chapter 16 Preparations of meat of fish of crustaceans molluscs or other aquatic invertebrates or of insects"@en-AU ;
    dct:isPartOf C2004A04997:103 ;
    rdfs:comment "Chapter 16 Preparations of meat of fish of crustaceans molluscs or other aquatic invertebrates or of insects - Abrievated Graph Key: C107"@en-AU ;
    rdfs:subClassOf C2004A04997: ;
    skos:definition "Chapter 16 Preparations of meat of fish of crustaceans molluscs or other aquatic invertebrates or of insects"@en-AU ;
    skos:narrower C2004A04997:103 ;
    skos:prefLabel "Chapter C107"@en-AU ;
    dcat:accessURL <https://www.legislation.gov.au/C2004A04997/2024-07-01/2024-07-01/text/1/epub/OEBPS/document_2/document_2.html#_Toc171750933> ;
    dcat:landingPage "https://www.legislation.gov.au/C2004A04997/2024-07-01/2024-07-01/text/1/epub/OEBPS/document_2/document_2.html#_Toc171750933"^^xsd:anyURI ;
    dcat:theme legcons:Chapter .

C2004A04997:108 a legcons:Item,
        C2004A04997:Item,
        owl:Class,
        dcat:Resource ;
    rdfs:label "Item - I108 Notes"@en-AU ;
    dct:isPartOf C2004A04997:103 ;
    rdfs:comment "Notes - Abrievated Graph Key: I108"@en-AU ;
    rdfs:subClassOf C2004A04997: ;
    skos:definition "Notes"@en-AU ;
    skos:narrower C2004A04997:103 ;
    skos:prefLabel "Item I108"@en-AU ;
    dcat:accessURL <https://www.legislation.gov.au/C2004A04997/2024-07-01/2024-07-01/text/1/epub/OEBPS/document_2/document_2.html#_Toc171750934> ;
    dcat:landingPage "https://www.legislation.gov.au/C2004A04997/2024-07-01/2024-07-01/text/1/epub/OEBPS/document_2/document_2.html#_Toc171750934"^^xsd:anyURI ;
    dcat:theme legcons:Item .

C2004A04997:109 a legcons:Item,
        C2004A04997:Item,
        owl:Class,
        dcat:Resource ;
    rdfs:label "Item - I109 Subheading Notes"@en-AU ;
    dct:isPartOf C2004A04997:103 ;
    rdfs:comment "Subheading Notes - Abrievated Graph Key: I109"@en-AU ;
    rdfs:subClassOf C2004A04997: ;
    skos:definition "Subheading Notes"@en-AU ;
    skos:narrower C2004A04997:103 ;
    skos:prefLabel "Item I109"@en-AU ;
    dcat:accessURL <https://www.legislation.gov.au/C2004A04997/2024-07-01/2024-07-01/text/1/epub/OEBPS/document_2/document_2.html#_Toc171750935> ;
    dcat:landingPage "https://www.legislation.gov.au/C2004A04997/2024-07-01/2024-07-01/text/1/epub/OEBPS/document_2/document_2.html#_Toc171750935"^^xsd:anyURI ;
    dcat:theme legcons:Item .

C2004A04997:11 a legcons:Item,
        C2004A04997:Item,
        owl:Class,
        dcat:Resource ;
    rdfs:label "Item - I11 8  Application of Schedule 4"@en-AU ;
    dct:isPartOf C2004A04997:2 ;
    rdfs:comment "8  Application of Schedule 4 - Abrievated Graph Key: I11"@en-AU ;
    rdfs:subClassOf C2004A04997: ;
    skos:definition "8  Application of Schedule 4"@en-AU ;
    skos:narrower C2004A04997:2 ;
    skos:prefLabel "Item I11"@en-AU ;
    dcat:accessURL <https://www.legislation.gov.au/C2004A04997/2024-07-01/2024-07-01/text/1/epub/OEBPS/document_1/document_1.html#_Toc172806511> ;
    dcat:landingPage "https://www.legislation.gov.au/C2004A04997/2024-07-01/2024-07-01/text/1/epub/OEBPS/document_1/document_1.html#_Toc172806511"^^xsd:anyURI ;
    dcat:theme legcons:Item .

C2004A04997:110 a legcons:Chapter,
        C2004A04997:Chapter,
        owl:Class,
        dcat:Resource ;
    rdfs:label "Chapter - C110 Chapter 17 Sugars and sugar confectionery"@en-AU ;
    dct:isPartOf C2004A04997:103 ;
    rdfs:comment "Chapter 17 Sugars and sugar confectionery - Abrievated Graph Key: C110"@en-AU ;
    rdfs:subClassOf C2004A04997: ;
    skos:definition "Chapter 17 Sugars and sugar confectionery"@en-AU ;
    skos:narrower C2004A04997:103 ;
    skos:prefLabel "Chapter C110"@en-AU ;
    dcat:accessURL <https://www.legislation.gov.au/C2004A04997/2024-07-01/2024-07-01/text/1/epub/OEBPS/document_2/document_2.html#_Toc171750936> ;
    dcat:landingPage "https://www.legislation.gov.au/C2004A04997/2024-07-01/2024-07-01/text/1/epub/OEBPS/document_2/document_2.html#_Toc171750936"^^xsd:anyURI ;
    dcat:theme legcons:Chapter .

C2004A04997:111 a legcons:Item,
        C2004A04997:Item,
        owl:Class,
        dcat:Resource ;
    rdfs:label "Item - I111 Note"@en-AU ;
    dct:isPartOf C2004A04997:103 ;
    rdfs:comment "Note - Abrievated Graph Key: I111"@en-AU ;
    rdfs:subClassOf C2004A04997: ;
    skos:definition "Note"@en-AU ;
    skos:narrower C2004A04997:103 ;
    skos:prefLabel "Item I111"@en-AU ;
    dcat:accessURL <https://www.legislation.gov.au/C2004A04997/2024-07-01/2024-07-01/text/1/epub/OEBPS/document_2/document_2.html#_Toc171750937> ;
    dcat:landingPage "https://www.legislation.gov.au/C2004A04997/2024-07-01/2024-07-01/text/1/epub/OEBPS/document_2/document_2.html#_Toc171750937"^^xsd:anyURI ;
    dcat:theme legcons:Item .

C2004A04997:112 a legcons:Item,
        C2004A04997:Item,
        owl:Class,
        dcat:Resource ;
    rdfs:label "Item - I112 Subheading Notes"@en-AU ;
    dct:isPartOf C2004A04997:103 ;
    rdfs:comment "Subheading Notes - Abrievated Graph Key: I112"@en-AU ;
    rdfs:subClassOf C2004A04997: ;
    skos:definition "Subheading Notes"@en-AU ;
    skos:narrower C2004A04997:103 ;
    skos:prefLabel "Item I112"@en-AU ;
    dcat:accessURL <https://www.legislation.gov.au/C2004A04997/2024-07-01/2024-07-01/text/1/epub/OEBPS/document_2/document_2.html#_Toc171750938> ;
    dcat:landingPage "https://www.legislation.gov.au/C2004A04997/2024-07-01/2024-07-01/text/1/epub/OEBPS/document_2/document_2.html#_Toc171750938"^^xsd:anyURI ;
    dcat:theme legcons:Item .

C2004A04997:113 a legcons:Chapter,
        C2004A04997:Chapter,
        owl:Class,
        dcat:Resource ;
    rdfs:label "Chapter - C113 Chapter 18 Cocoa and cocoa preparations"@en-AU ;
    dct:isPartOf C2004A04997:103 ;
    rdfs:comment "Chapter 18 Cocoa and cocoa preparations - Abrievated Graph Key: C113"@en-AU ;
    rdfs:subClassOf C2004A04997: ;
    skos:definition "Chapter 18 Cocoa and cocoa preparations"@en-AU ;
    skos:narrower C2004A04997:103 ;
    skos:prefLabel "Chapter C113"@en-AU ;
    dcat:accessURL <https://www.legislation.gov.au/C2004A04997/2024-07-01/2024-07-01/text/1/epub/OEBPS/document_2/document_2.html#_Toc171750939> ;
    dcat:landingPage "https://www.legislation.gov.au/C2004A04997/2024-07-01/2024-07-01/text/1/epub/OEBPS/document_2/document_2.html#_Toc171750939"^^xsd:anyURI ;
    dcat:theme legcons:Chapter .

C2004A04997:114 a legcons:Item,
        C2004A04997:Item,
        owl:Class,
        dcat:Resource ;
    rdfs:label "Item - I114 Notes"@en-AU ;
    dct:isPartOf C2004A04997:103 ;
    rdfs:comment "Notes - Abrievated Graph Key: I114"@en-AU ;
    rdfs:subClassOf C2004A04997: ;
    skos:definition "Notes"@en-AU ;
    skos:narrower C2004A04997:103 ;
    skos:prefLabel "Item I114"@en-AU ;
    dcat:accessURL <https://www.legislation.gov.au/C2004A04997/2024-07-01/2024-07-01/text/1/epub/OEBPS/document_2/document_2.html#_Toc171750940> ;
    dcat:landingPage "https://www.legislation.gov.au/C2004A04997/2024-07-01/2024-07-01/text/1/epub/OEBPS/document_2/document_2.html#_Toc171750940"^^xsd:anyURI ;
    dcat:theme legcons:Item .

C2004A04997:115 a legcons:Chapter,
        C2004A04997:Chapter,
        owl:Class,
        dcat:Resource ;
    rdfs:label "Chapter - C115 Chapter 19 Preparations of cereals flour starch or milk pastrycooks products"@en-AU ;
    dct:isPartOf C2004A04997:103 ;
    rdfs:comment "Chapter 19 Preparations of cereals flour starch or milk pastrycooks products - Abrievated Graph Key: C115"@en-AU ;
    rdfs:subClassOf C2004A04997: ;
    skos:definition "Chapter 19 Preparations of cereals flour starch or milk pastrycooks products"@en-AU ;
    skos:narrower C2004A04997:103 ;
    skos:prefLabel "Chapter C115"@en-AU ;
    dcat:accessURL <https://www.legislation.gov.au/C2004A04997/2024-07-01/2024-07-01/text/1/epub/OEBPS/document_2/document_2.html#_Toc171750941> ;
    dcat:landingPage "https://www.legislation.gov.au/C2004A04997/2024-07-01/2024-07-01/text/1/epub/OEBPS/document_2/document_2.html#_Toc171750941"^^xsd:anyURI ;
    dcat:theme legcons:Chapter .

C2004A04997:116 a legcons:Item,
        C2004A04997:Item,
        owl:Class,
        dcat:Resource ;
    rdfs:label "Item - I116 Notes"@en-AU ;
    dct:isPartOf C2004A04997:103 ;
    rdfs:comment "Notes - Abrievated Graph Key: I116"@en-AU ;
    rdfs:subClassOf C2004A04997: ;
    skos:definition "Notes"@en-AU ;
    skos:narrower C2004A04997:103 ;
    skos:prefLabel "Item I116"@en-AU ;
    dcat:accessURL <https://www.legislation.gov.au/C2004A04997/2024-07-01/2024-07-01/text/1/epub/OEBPS/document_2/document_2.html#_Toc171750942> ;
    dcat:landingPage "https://www.legislation.gov.au/C2004A04997/2024-07-01/2024-07-01/text/1/epub/OEBPS/document_2/document_2.html#_Toc171750942"^^xsd:anyURI ;
    dcat:theme legcons:Item .

C2004A04997:117 a legcons:Item,
        C2004A04997:Item,
        owl:Class,
        dcat:Resource ;
    rdfs:label "Item - I117 Additional Note"@en-AU ;
    dct:isPartOf C2004A04997:103 ;
    rdfs:comment "Additional Note - Abrievated Graph Key: I117"@en-AU ;
    rdfs:subClassOf C2004A04997: ;
    skos:definition "Additional Note"@en-AU ;
    skos:narrower C2004A04997:103 ;
    skos:prefLabel "Item I117"@en-AU ;
    dcat:accessURL <https://www.legislation.gov.au/C2004A04997/2024-07-01/2024-07-01/text/1/epub/OEBPS/document_2/document_2.html#_Toc171750943> ;
    dcat:landingPage "https://www.legislation.gov.au/C2004A04997/2024-07-01/2024-07-01/text/1/epub/OEBPS/document_2/document_2.html#_Toc171750943"^^xsd:anyURI ;
    dcat:theme legcons:Item .

C2004A04997:118 a legcons:Chapter,
        C2004A04997:Chapter,
        owl:Class,
        dcat:Resource ;
    rdfs:label "Chapter - C118 Chapter 20 Preparations of vegetables fruit nuts or other parts of plants"@en-AU ;
    dct:isPartOf C2004A04997:103 ;
    rdfs:comment "Chapter 20 Preparations of vegetables fruit nuts or other parts of plants - Abrievated Graph Key: C118"@en-AU ;
    rdfs:subClassOf C2004A04997: ;
    skos:definition "Chapter 20 Preparations of vegetables fruit nuts or other parts of plants"@en-AU ;
    skos:narrower C2004A04997:103 ;
    skos:prefLabel "Chapter C118"@en-AU ;
    dcat:accessURL <https://www.legislation.gov.au/C2004A04997/2024-07-01/2024-07-01/text/1/epub/OEBPS/document_2/document_2.html#_Toc171750944> ;
    dcat:landingPage "https://www.legislation.gov.au/C2004A04997/2024-07-01/2024-07-01/text/1/epub/OEBPS/document_2/document_2.html#_Toc171750944"^^xsd:anyURI ;
    dcat:theme legcons:Chapter .

C2004A04997:119 a legcons:Item,
        C2004A04997:Item,
        owl:Class,
        dcat:Resource ;
    rdfs:label "Item - I119 Notes"@en-AU ;
    dct:isPartOf C2004A04997:103 ;
    rdfs:comment "Notes - Abrievated Graph Key: I119"@en-AU ;
    rdfs:subClassOf C2004A04997: ;
    skos:definition "Notes"@en-AU ;
    skos:narrower C2004A04997:103 ;
    skos:prefLabel "Item I119"@en-AU ;
    dcat:accessURL <https://www.legislation.gov.au/C2004A04997/2024-07-01/2024-07-01/text/1/epub/OEBPS/document_2/document_2.html#_Toc171750945> ;
    dcat:landingPage "https://www.legislation.gov.au/C2004A04997/2024-07-01/2024-07-01/text/1/epub/OEBPS/document_2/document_2.html#_Toc171750945"^^xsd:anyURI ;
    dcat:theme legcons:Item .

C2004A04997:12 a legcons:Item,
        C2004A04997:Item,
        owl:Class,
        dcat:Resource ;
    rdfs:label "Item - I12 9  Rates of dutyad valorem duties"@en-AU ;
    dct:isPartOf C2004A04997:2 ;
    rdfs:comment "9  Rates of dutyad valorem duties - Abrievated Graph Key: I12"@en-AU ;
    rdfs:subClassOf C2004A04997: ;
    skos:definition "9  Rates of dutyad valorem duties"@en-AU ;
    skos:narrower C2004A04997:2 ;
    skos:prefLabel "Item I12"@en-AU ;
    dcat:accessURL <https://www.legislation.gov.au/C2004A04997/2024-07-01/2024-07-01/text/1/epub/OEBPS/document_1/document_1.html#_Toc172806512> ;
    dcat:landingPage "https://www.legislation.gov.au/C2004A04997/2024-07-01/2024-07-01/text/1/epub/OEBPS/document_1/document_1.html#_Toc172806512"^^xsd:anyURI ;
    dcat:theme legcons:Item .

C2004A04997:120 a legcons:Item,
        C2004A04997:Item,
        owl:Class,
        dcat:Resource ;
    rdfs:label "Item - I120 Subheading Notes"@en-AU ;
    dct:isPartOf C2004A04997:103 ;
    rdfs:comment "Subheading Notes - Abrievated Graph Key: I120"@en-AU ;
    rdfs:subClassOf C2004A04997: ;
    skos:definition "Subheading Notes"@en-AU ;
    skos:narrower C2004A04997:103 ;
    skos:prefLabel "Item I120"@en-AU ;
    dcat:accessURL <https://www.legislation.gov.au/C2004A04997/2024-07-01/2024-07-01/text/1/epub/OEBPS/document_2/document_2.html#_Toc171750946> ;
    dcat:landingPage "https://www.legislation.gov.au/C2004A04997/2024-07-01/2024-07-01/text/1/epub/OEBPS/document_2/document_2.html#_Toc171750946"^^xsd:anyURI ;
    dcat:theme legcons:Item .

C2004A04997:121 a legcons:Item,
        C2004A04997:Item,
        owl:Class,
        dcat:Resource ;
    rdfs:label "Item - I121 Additional Notes"@en-AU ;
    dct:isPartOf C2004A04997:103 ;
    rdfs:comment "Additional Notes - Abrievated Graph Key: I121"@en-AU ;
    rdfs:subClassOf C2004A04997: ;
    skos:definition "Additional Notes"@en-AU ;
    skos:narrower C2004A04997:103 ;
    skos:prefLabel "Item I121"@en-AU ;
    dcat:accessURL <https://www.legislation.gov.au/C2004A04997/2024-07-01/2024-07-01/text/1/epub/OEBPS/document_2/document_2.html#_Toc171750947> ;
    dcat:landingPage "https://www.legislation.gov.au/C2004A04997/2024-07-01/2024-07-01/text/1/epub/OEBPS/document_2/document_2.html#_Toc171750947"^^xsd:anyURI ;
    dcat:theme legcons:Item .

C2004A04997:122 a legcons:Chapter,
        C2004A04997:Chapter,
        owl:Class,
        dcat:Resource ;
    rdfs:label "Chapter - C122 Chapter 21 Miscellaneous edible preparations"@en-AU ;
    dct:isPartOf C2004A04997:103 ;
    rdfs:comment "Chapter 21 Miscellaneous edible preparations - Abrievated Graph Key: C122"@en-AU ;
    rdfs:subClassOf C2004A04997: ;
    skos:definition "Chapter 21 Miscellaneous edible preparations"@en-AU ;
    skos:narrower C2004A04997:103 ;
    skos:prefLabel "Chapter C122"@en-AU ;
    dcat:accessURL <https://www.legislation.gov.au/C2004A04997/2024-07-01/2024-07-01/text/1/epub/OEBPS/document_2/document_2.html#_Toc171750948> ;
    dcat:landingPage "https://www.legislation.gov.au/C2004A04997/2024-07-01/2024-07-01/text/1/epub/OEBPS/document_2/document_2.html#_Toc171750948"^^xsd:anyURI ;
    dcat:theme legcons:Chapter .

C2004A04997:123 a legcons:Item,
        C2004A04997:Item,
        owl:Class,
        dcat:Resource ;
    rdfs:label "Item - I123 Notes"@en-AU ;
    dct:isPartOf C2004A04997:103 ;
    rdfs:comment "Notes - Abrievated Graph Key: I123"@en-AU ;
    rdfs:subClassOf C2004A04997: ;
    skos:definition "Notes"@en-AU ;
    skos:narrower C2004A04997:103 ;
    skos:prefLabel "Item I123"@en-AU ;
    dcat:accessURL <https://www.legislation.gov.au/C2004A04997/2024-07-01/2024-07-01/text/1/epub/OEBPS/document_2/document_2.html#_Toc171750949> ;
    dcat:landingPage "https://www.legislation.gov.au/C2004A04997/2024-07-01/2024-07-01/text/1/epub/OEBPS/document_2/document_2.html#_Toc171750949"^^xsd:anyURI ;
    dcat:theme legcons:Item .

C2004A04997:124 a legcons:Item,
        C2004A04997:Item,
        owl:Class,
        dcat:Resource ;
    rdfs:label "Item - I124 Additional Notes"@en-AU ;
    dct:isPartOf C2004A04997:103 ;
    rdfs:comment "Additional Notes - Abrievated Graph Key: I124"@en-AU ;
    rdfs:subClassOf C2004A04997: ;
    skos:definition "Additional Notes"@en-AU ;
    skos:narrower C2004A04997:103 ;
    skos:prefLabel "Item I124"@en-AU ;
    dcat:accessURL <https://www.legislation.gov.au/C2004A04997/2024-07-01/2024-07-01/text/1/epub/OEBPS/document_2/document_2.html#_Toc171750950> ;
    dcat:landingPage "https://www.legislation.gov.au/C2004A04997/2024-07-01/2024-07-01/text/1/epub/OEBPS/document_2/document_2.html#_Toc171750950"^^xsd:anyURI ;
    dcat:theme legcons:Item .

C2004A04997:125 a legcons:Chapter,
        C2004A04997:Chapter,
        owl:Class,
        dcat:Resource ;
    rdfs:label "Chapter - C125 Chapter 22 Beverages spirits and vinegar"@en-AU ;
    dct:isPartOf C2004A04997:103 ;
    rdfs:comment "Chapter 22 Beverages spirits and vinegar - Abrievated Graph Key: C125"@en-AU ;
    rdfs:subClassOf C2004A04997: ;
    skos:definition "Chapter 22 Beverages spirits and vinegar"@en-AU ;
    skos:narrower C2004A04997:103 ;
    skos:prefLabel "Chapter C125"@en-AU ;
    dcat:accessURL <https://www.legislation.gov.au/C2004A04997/2024-07-01/2024-07-01/text/1/epub/OEBPS/document_2/document_2.html#_Toc171750951> ;
    dcat:landingPage "https://www.legislation.gov.au/C2004A04997/2024-07-01/2024-07-01/text/1/epub/OEBPS/document_2/document_2.html#_Toc171750951"^^xsd:anyURI ;
    dcat:theme legcons:Chapter .

C2004A04997:126 a legcons:Item,
        C2004A04997:Item,
        owl:Class,
        dcat:Resource ;
    rdfs:label "Item - I126 Notes"@en-AU ;
    dct:isPartOf C2004A04997:103 ;
    rdfs:comment "Notes - Abrievated Graph Key: I126"@en-AU ;
    rdfs:subClassOf C2004A04997: ;
    skos:definition "Notes"@en-AU ;
    skos:narrower C2004A04997:103 ;
    skos:prefLabel "Item I126"@en-AU ;
    dcat:accessURL <https://www.legislation.gov.au/C2004A04997/2024-07-01/2024-07-01/text/1/epub/OEBPS/document_2/document_2.html#_Toc171750952> ;
    dcat:landingPage "https://www.legislation.gov.au/C2004A04997/2024-07-01/2024-07-01/text/1/epub/OEBPS/document_2/document_2.html#_Toc171750952"^^xsd:anyURI ;
    dcat:theme legcons:Item .

C2004A04997:127 a legcons:Item,
        C2004A04997:Item,
        owl:Class,
        dcat:Resource ;
    rdfs:label "Item - I127 Subheading Note"@en-AU ;
    dct:isPartOf C2004A04997:103 ;
    rdfs:comment "Subheading Note - Abrievated Graph Key: I127"@en-AU ;
    rdfs:subClassOf C2004A04997: ;
    skos:definition "Subheading Note"@en-AU ;
    skos:narrower C2004A04997:103 ;
    skos:prefLabel "Item I127"@en-AU ;
    dcat:accessURL <https://www.legislation.gov.au/C2004A04997/2024-07-01/2024-07-01/text/1/epub/OEBPS/document_2/document_2.html#_Toc171750953> ;
    dcat:landingPage "https://www.legislation.gov.au/C2004A04997/2024-07-01/2024-07-01/text/1/epub/OEBPS/document_2/document_2.html#_Toc171750953"^^xsd:anyURI ;
    dcat:theme legcons:Item .

C2004A04997:128 a legcons:Item,
        C2004A04997:Item,
        owl:Class,
        dcat:Resource ;
    rdfs:label "Item - I128 Additional Notes"@en-AU ;
    dct:isPartOf C2004A04997:103 ;
    rdfs:comment "Additional Notes - Abrievated Graph Key: I128"@en-AU ;
    rdfs:subClassOf C2004A04997: ;
    skos:definition "Additional Notes"@en-AU ;
    skos:narrower C2004A04997:103 ;
    skos:prefLabel "Item I128"@en-AU ;
    dcat:accessURL <https://www.legislation.gov.au/C2004A04997/2024-07-01/2024-07-01/text/1/epub/OEBPS/document_2/document_2.html#_Toc171750954> ;
    dcat:landingPage "https://www.legislation.gov.au/C2004A04997/2024-07-01/2024-07-01/text/1/epub/OEBPS/document_2/document_2.html#_Toc171750954"^^xsd:anyURI ;
    dcat:theme legcons:Item .

C2004A04997:129 a legcons:Chapter,
        C2004A04997:Chapter,
        owl:Class,
        dcat:Resource ;
    rdfs:label "Chapter - C129 Chapter 23 Residues and waste from the food industries prepared animal fodder"@en-AU ;
    dct:isPartOf C2004A04997:103 ;
    rdfs:comment "Chapter 23 Residues and waste from the food industries prepared animal fodder - Abrievated Graph Key: C129"@en-AU ;
    rdfs:subClassOf C2004A04997: ;
    skos:definition "Chapter 23 Residues and waste from the food industries prepared animal fodder"@en-AU ;
    skos:narrower C2004A04997:103 ;
    skos:prefLabel "Chapter C129"@en-AU ;
    dcat:accessURL <https://www.legislation.gov.au/C2004A04997/2024-07-01/2024-07-01/text/1/epub/OEBPS/document_2/document_2.html#_Toc171750955> ;
    dcat:landingPage "https://www.legislation.gov.au/C2004A04997/2024-07-01/2024-07-01/text/1/epub/OEBPS/document_2/document_2.html#_Toc171750955"^^xsd:anyURI ;
    dcat:theme legcons:Chapter .

C2004A04997:13 a legcons:Item,
        C2004A04997:Item,
        owl:Class,
        dcat:Resource ;
    rdfs:label "Item - I13 10  Certain words etc are rates of duty"@en-AU ;
    dct:isPartOf C2004A04997:2 ;
    rdfs:comment "10  Certain words etc are rates of duty - Abrievated Graph Key: I13"@en-AU ;
    rdfs:subClassOf C2004A04997: ;
    skos:definition "10  Certain words etc are rates of duty"@en-AU ;
    skos:narrower C2004A04997:2 ;
    skos:prefLabel "Item I13"@en-AU ;
    dcat:accessURL <https://www.legislation.gov.au/C2004A04997/2024-07-01/2024-07-01/text/1/epub/OEBPS/document_1/document_1.html#_Toc172806513> ;
    dcat:landingPage "https://www.legislation.gov.au/C2004A04997/2024-07-01/2024-07-01/text/1/epub/OEBPS/document_1/document_1.html#_Toc172806513"^^xsd:anyURI ;
    dcat:theme legcons:Item .

C2004A04997:130 a legcons:Item,
        C2004A04997:Item,
        owl:Class,
        dcat:Resource ;
    rdfs:label "Item - I130 Note"@en-AU ;
    dct:isPartOf C2004A04997:103 ;
    rdfs:comment "Note - Abrievated Graph Key: I130"@en-AU ;
    rdfs:subClassOf C2004A04997: ;
    skos:definition "Note"@en-AU ;
    skos:narrower C2004A04997:103 ;
    skos:prefLabel "Item I130"@en-AU ;
    dcat:accessURL <https://www.legislation.gov.au/C2004A04997/2024-07-01/2024-07-01/text/1/epub/OEBPS/document_2/document_2.html#_Toc171750956> ;
    dcat:landingPage "https://www.legislation.gov.au/C2004A04997/2024-07-01/2024-07-01/text/1/epub/OEBPS/document_2/document_2.html#_Toc171750956"^^xsd:anyURI ;
    dcat:theme legcons:Item .

C2004A04997:131 a legcons:Item,
        C2004A04997:Item,
        owl:Class,
        dcat:Resource ;
    rdfs:label "Item - I131 Subheading Note"@en-AU ;
    dct:isPartOf C2004A04997:103 ;
    rdfs:comment "Subheading Note - Abrievated Graph Key: I131"@en-AU ;
    rdfs:subClassOf C2004A04997: ;
    skos:definition "Subheading Note"@en-AU ;
    skos:narrower C2004A04997:103 ;
    skos:prefLabel "Item I131"@en-AU ;
    dcat:accessURL <https://www.legislation.gov.au/C2004A04997/2024-07-01/2024-07-01/text/1/epub/OEBPS/document_2/document_2.html#_Toc171750957> ;
    dcat:landingPage "https://www.legislation.gov.au/C2004A04997/2024-07-01/2024-07-01/text/1/epub/OEBPS/document_2/document_2.html#_Toc171750957"^^xsd:anyURI ;
    dcat:theme legcons:Item .

C2004A04997:132 a legcons:Chapter,
        C2004A04997:Chapter,
        owl:Class,
        dcat:Resource ;
    rdfs:label "Chapter - C132 Chapter 24 Tobacco and manufactured tobacco substitutes products whether or not containing nicotine intended for inhalation without combustion other nicotine containing products intended for the intake of nicotine into the human body"@en-AU ;
    dct:isPartOf C2004A04997:103 ;
    rdfs:comment "Chapter 24 Tobacco and manufactured tobacco substitutes products whether or not containing nicotine intended for inhalation without combustion other nicotine containing products intended for the intake of nicotine into the human body - Abrievated Graph Key: C132"@en-AU ;
    rdfs:subClassOf C2004A04997: ;
    skos:definition "Chapter 24 Tobacco and manufactured tobacco substitutes products whether or not containing nicotine intended for inhalation without combustion other nicotine containing products intended for the intake of nicotine into the human body"@en-AU ;
    skos:narrower C2004A04997:103 ;
    skos:prefLabel "Chapter C132"@en-AU ;
    dcat:accessURL <https://www.legislation.gov.au/C2004A04997/2024-07-01/2024-07-01/text/1/epub/OEBPS/document_2/document_2.html#_Toc171750958> ;
    dcat:landingPage "https://www.legislation.gov.au/C2004A04997/2024-07-01/2024-07-01/text/1/epub/OEBPS/document_2/document_2.html#_Toc171750958"^^xsd:anyURI ;
    dcat:theme legcons:Chapter .

C2004A04997:133 a legcons:Item,
        C2004A04997:Item,
        owl:Class,
        dcat:Resource ;
    rdfs:label "Item - I133 Notes"@en-AU ;
    dct:isPartOf C2004A04997:103 ;
    rdfs:comment "Notes - Abrievated Graph Key: I133"@en-AU ;
    rdfs:subClassOf C2004A04997: ;
    skos:definition "Notes"@en-AU ;
    skos:narrower C2004A04997:103 ;
    skos:prefLabel "Item I133"@en-AU ;
    dcat:accessURL <https://www.legislation.gov.au/C2004A04997/2024-07-01/2024-07-01/text/1/epub/OEBPS/document_2/document_2.html#_Toc171750959> ;
    dcat:landingPage "https://www.legislation.gov.au/C2004A04997/2024-07-01/2024-07-01/text/1/epub/OEBPS/document_2/document_2.html#_Toc171750959"^^xsd:anyURI ;
    dcat:theme legcons:Item .

C2004A04997:134 a legcons:Item,
        C2004A04997:Item,
        owl:Class,
        dcat:Resource ;
    rdfs:label "Item - I134 Subheading Note"@en-AU ;
    dct:isPartOf C2004A04997:103 ;
    rdfs:comment "Subheading Note - Abrievated Graph Key: I134"@en-AU ;
    rdfs:subClassOf C2004A04997: ;
    skos:definition "Subheading Note"@en-AU ;
    skos:narrower C2004A04997:103 ;
    skos:prefLabel "Item I134"@en-AU ;
    dcat:accessURL <https://www.legislation.gov.au/C2004A04997/2024-07-01/2024-07-01/text/1/epub/OEBPS/document_2/document_2.html#_Toc171750960> ;
    dcat:landingPage "https://www.legislation.gov.au/C2004A04997/2024-07-01/2024-07-01/text/1/epub/OEBPS/document_2/document_2.html#_Toc171750960"^^xsd:anyURI ;
    dcat:theme legcons:Item .

C2004A04997:135 a legcons:Item,
        C2004A04997:Item,
        owl:Class,
        dcat:Resource ;
    rdfs:label "Item - I135 Additional Notes"@en-AU ;
    dct:isPartOf C2004A04997:103 ;
    rdfs:comment "Additional Notes - Abrievated Graph Key: I135"@en-AU ;
    rdfs:subClassOf C2004A04997: ;
    skos:definition "Additional Notes"@en-AU ;
    skos:narrower C2004A04997:103 ;
    skos:prefLabel "Item I135"@en-AU ;
    dcat:accessURL <https://www.legislation.gov.au/C2004A04997/2024-07-01/2024-07-01/text/1/epub/OEBPS/document_2/document_2.html#_Toc171750961> ;
    dcat:landingPage "https://www.legislation.gov.au/C2004A04997/2024-07-01/2024-07-01/text/1/epub/OEBPS/document_2/document_2.html#_Toc171750961"^^xsd:anyURI ;
    dcat:theme legcons:Item .

C2004A04997:136 a legcons:Section,
        C2004A04997:Section,
        owl:Class,
        dcat:Resource ;
    rdfs:label "Section - S136 Section VMineral products"@en-AU ;
    dct:isPartOf C2004A04997:103 ;
    rdfs:comment "Section VMineral products - Abrievated Graph Key: S136"@en-AU ;
    rdfs:subClassOf C2004A04997: ;
    skos:definition "Section VMineral products"@en-AU ;
    skos:narrower C2004A04997:103 ;
    skos:prefLabel "Section S136"@en-AU ;
    dcat:accessURL <https://www.legislation.gov.au/C2004A04997/2024-07-01/2024-07-01/text/1/epub/OEBPS/document_2/document_2.html#_Toc171750962> ;
    dcat:landingPage "https://www.legislation.gov.au/C2004A04997/2024-07-01/2024-07-01/text/1/epub/OEBPS/document_2/document_2.html#_Toc171750962"^^xsd:anyURI ;
    dcat:theme legcons:Section .

C2004A04997:137 a legcons:Chapter,
        C2004A04997:Chapter,
        owl:Class,
        dcat:Resource ;
    rdfs:label "Chapter - C137 Chapter 25 Salt sulphur earths and stone plastering materials lime and cement"@en-AU ;
    dct:isPartOf C2004A04997:103 ;
    rdfs:comment "Chapter 25 Salt sulphur earths and stone plastering materials lime and cement - Abrievated Graph Key: C137"@en-AU ;
    rdfs:subClassOf C2004A04997: ;
    skos:definition "Chapter 25 Salt sulphur earths and stone plastering materials lime and cement"@en-AU ;
    skos:narrower C2004A04997:103 ;
    skos:prefLabel "Chapter C137"@en-AU ;
    dcat:accessURL <https://www.legislation.gov.au/C2004A04997/2024-07-01/2024-07-01/text/1/epub/OEBPS/document_2/document_2.html#_Toc171750963> ;
    dcat:landingPage "https://www.legislation.gov.au/C2004A04997/2024-07-01/2024-07-01/text/1/epub/OEBPS/document_2/document_2.html#_Toc171750963"^^xsd:anyURI ;
    dcat:theme legcons:Chapter .

C2004A04997:138 a legcons:Item,
        C2004A04997:Item,
        owl:Class,
        dcat:Resource ;
    rdfs:label "Item - I138 Notes"@en-AU ;
    dct:isPartOf C2004A04997:103 ;
    rdfs:comment "Notes - Abrievated Graph Key: I138"@en-AU ;
    rdfs:subClassOf C2004A04997: ;
    skos:definition "Notes"@en-AU ;
    skos:narrower C2004A04997:103 ;
    skos:prefLabel "Item I138"@en-AU ;
    dcat:accessURL <https://www.legislation.gov.au/C2004A04997/2024-07-01/2024-07-01/text/1/epub/OEBPS/document_2/document_2.html#_Toc171750964> ;
    dcat:landingPage "https://www.legislation.gov.au/C2004A04997/2024-07-01/2024-07-01/text/1/epub/OEBPS/document_2/document_2.html#_Toc171750964"^^xsd:anyURI ;
    dcat:theme legcons:Item .

C2004A04997:139 a legcons:Chapter,
        C2004A04997:Chapter,
        owl:Class,
        dcat:Resource ;
    rdfs:label "Chapter - C139 Chapter 26 Ores slag and ash"@en-AU ;
    dct:isPartOf C2004A04997:103 ;
    rdfs:comment "Chapter 26 Ores slag and ash - Abrievated Graph Key: C139"@en-AU ;
    rdfs:subClassOf C2004A04997: ;
    skos:definition "Chapter 26 Ores slag and ash"@en-AU ;
    skos:narrower C2004A04997:103 ;
    skos:prefLabel "Chapter C139"@en-AU ;
    dcat:accessURL <https://www.legislation.gov.au/C2004A04997/2024-07-01/2024-07-01/text/1/epub/OEBPS/document_2/document_2.html#_Toc171750965> ;
    dcat:landingPage "https://www.legislation.gov.au/C2004A04997/2024-07-01/2024-07-01/text/1/epub/OEBPS/document_2/document_2.html#_Toc171750965"^^xsd:anyURI ;
    dcat:theme legcons:Chapter .

C2004A04997:14 a legcons:Item,
        C2004A04997:Item,
        owl:Class,
        dcat:Resource ;
    rdfs:label "Item - I14 11  Rates of dutyphasing rates"@en-AU ;
    dct:isPartOf C2004A04997:2 ;
    rdfs:comment "11  Rates of dutyphasing rates - Abrievated Graph Key: I14"@en-AU ;
    rdfs:subClassOf C2004A04997: ;
    skos:definition "11  Rates of dutyphasing rates"@en-AU ;
    skos:narrower C2004A04997:2 ;
    skos:prefLabel "Item I14"@en-AU ;
    dcat:accessURL <https://www.legislation.gov.au/C2004A04997/2024-07-01/2024-07-01/text/1/epub/OEBPS/document_1/document_1.html#_Toc172806514> ;
    dcat:landingPage "https://www.legislation.gov.au/C2004A04997/2024-07-01/2024-07-01/text/1/epub/OEBPS/document_1/document_1.html#_Toc172806514"^^xsd:anyURI ;
    dcat:theme legcons:Item .

C2004A04997:140 a legcons:Item,
        C2004A04997:Item,
        owl:Class,
        dcat:Resource ;
    rdfs:label "Item - I140 Notes"@en-AU ;
    dct:isPartOf C2004A04997:103 ;
    rdfs:comment "Notes - Abrievated Graph Key: I140"@en-AU ;
    rdfs:subClassOf C2004A04997: ;
    skos:definition "Notes"@en-AU ;
    skos:narrower C2004A04997:103 ;
    skos:prefLabel "Item I140"@en-AU ;
    dcat:accessURL <https://www.legislation.gov.au/C2004A04997/2024-07-01/2024-07-01/text/1/epub/OEBPS/document_2/document_2.html#_Toc171750966> ;
    dcat:landingPage "https://www.legislation.gov.au/C2004A04997/2024-07-01/2024-07-01/text/1/epub/OEBPS/document_2/document_2.html#_Toc171750966"^^xsd:anyURI ;
    dcat:theme legcons:Item .

C2004A04997:141 a legcons:Item,
        C2004A04997:Item,
        owl:Class,
        dcat:Resource ;
    rdfs:label "Item - I141 Subheading Notes"@en-AU ;
    dct:isPartOf C2004A04997:103 ;
    rdfs:comment "Subheading Notes - Abrievated Graph Key: I141"@en-AU ;
    rdfs:subClassOf C2004A04997: ;
    skos:definition "Subheading Notes"@en-AU ;
    skos:narrower C2004A04997:103 ;
    skos:prefLabel "Item I141"@en-AU ;
    dcat:accessURL <https://www.legislation.gov.au/C2004A04997/2024-07-01/2024-07-01/text/1/epub/OEBPS/document_2/document_2.html#_Toc171750967> ;
    dcat:landingPage "https://www.legislation.gov.au/C2004A04997/2024-07-01/2024-07-01/text/1/epub/OEBPS/document_2/document_2.html#_Toc171750967"^^xsd:anyURI ;
    dcat:theme legcons:Item .

C2004A04997:142 a legcons:Chapter,
        C2004A04997:Chapter,
        owl:Class,
        dcat:Resource ;
    rdfs:label "Chapter - C142 Chapter 27 Mineral fuels mineral oils and products of their distillation bituminous substances mineral waxes"@en-AU ;
    dct:isPartOf C2004A04997:103 ;
    rdfs:comment "Chapter 27 Mineral fuels mineral oils and products of their distillation bituminous substances mineral waxes - Abrievated Graph Key: C142"@en-AU ;
    rdfs:subClassOf C2004A04997: ;
    skos:definition "Chapter 27 Mineral fuels mineral oils and products of their distillation bituminous substances mineral waxes"@en-AU ;
    skos:narrower C2004A04997:103 ;
    skos:prefLabel "Chapter C142"@en-AU ;
    dcat:accessURL <https://www.legislation.gov.au/C2004A04997/2024-07-01/2024-07-01/text/1/epub/OEBPS/document_2/document_2.html#_Toc171750968> ;
    dcat:landingPage "https://www.legislation.gov.au/C2004A04997/2024-07-01/2024-07-01/text/1/epub/OEBPS/document_2/document_2.html#_Toc171750968"^^xsd:anyURI ;
    dcat:theme legcons:Chapter .

C2004A04997:143 a legcons:Item,
        C2004A04997:Item,
        owl:Class,
        dcat:Resource ;
    rdfs:label "Item - I143 Notes"@en-AU ;
    dct:isPartOf C2004A04997:103 ;
    rdfs:comment "Notes - Abrievated Graph Key: I143"@en-AU ;
    rdfs:subClassOf C2004A04997: ;
    skos:definition "Notes"@en-AU ;
    skos:narrower C2004A04997:103 ;
    skos:prefLabel "Item I143"@en-AU ;
    dcat:accessURL <https://www.legislation.gov.au/C2004A04997/2024-07-01/2024-07-01/text/1/epub/OEBPS/document_2/document_2.html#_Toc171750969> ;
    dcat:landingPage "https://www.legislation.gov.au/C2004A04997/2024-07-01/2024-07-01/text/1/epub/OEBPS/document_2/document_2.html#_Toc171750969"^^xsd:anyURI ;
    dcat:theme legcons:Item .

C2004A04997:144 a legcons:Item,
        C2004A04997:Item,
        owl:Class,
        dcat:Resource ;
    rdfs:label "Item - I144 Subheading Notes"@en-AU ;
    dct:isPartOf C2004A04997:103 ;
    rdfs:comment "Subheading Notes - Abrievated Graph Key: I144"@en-AU ;
    rdfs:subClassOf C2004A04997: ;
    skos:definition "Subheading Notes"@en-AU ;
    skos:narrower C2004A04997:103 ;
    skos:prefLabel "Item I144"@en-AU ;
    dcat:accessURL <https://www.legislation.gov.au/C2004A04997/2024-07-01/2024-07-01/text/1/epub/OEBPS/document_2/document_2.html#_Toc171750970> ;
    dcat:landingPage "https://www.legislation.gov.au/C2004A04997/2024-07-01/2024-07-01/text/1/epub/OEBPS/document_2/document_2.html#_Toc171750970"^^xsd:anyURI ;
    dcat:theme legcons:Item .

C2004A04997:145 a legcons:Item,
        C2004A04997:Item,
        owl:Class,
        dcat:Resource ;
    rdfs:label "Item - I145 Additional Notes"@en-AU ;
    dct:isPartOf C2004A04997:103 ;
    rdfs:comment "Additional Notes - Abrievated Graph Key: I145"@en-AU ;
    rdfs:subClassOf C2004A04997: ;
    skos:definition "Additional Notes"@en-AU ;
    skos:narrower C2004A04997:103 ;
    skos:prefLabel "Item I145"@en-AU ;
    dcat:accessURL <https://www.legislation.gov.au/C2004A04997/2024-07-01/2024-07-01/text/1/epub/OEBPS/document_2/document_2.html#_Toc171750971> ;
    dcat:landingPage "https://www.legislation.gov.au/C2004A04997/2024-07-01/2024-07-01/text/1/epub/OEBPS/document_2/document_2.html#_Toc171750971"^^xsd:anyURI ;
    dcat:theme legcons:Item .

C2004A04997:146 a legcons:Section,
        C2004A04997:Section,
        owl:Class,
        dcat:Resource ;
    rdfs:label "Section - S146 Section VIProducts of the chemical or allied industries"@en-AU ;
    dct:isPartOf C2004A04997:103 ;
    rdfs:comment "Section VIProducts of the chemical or allied industries - Abrievated Graph Key: S146"@en-AU ;
    rdfs:subClassOf C2004A04997: ;
    skos:definition "Section VIProducts of the chemical or allied industries"@en-AU ;
    skos:narrower C2004A04997:103 ;
    skos:prefLabel "Section S146"@en-AU ;
    dcat:accessURL <https://www.legislation.gov.au/C2004A04997/2024-07-01/2024-07-01/text/1/epub/OEBPS/document_2/document_2.html#_Toc171750972> ;
    dcat:landingPage "https://www.legislation.gov.au/C2004A04997/2024-07-01/2024-07-01/text/1/epub/OEBPS/document_2/document_2.html#_Toc171750972"^^xsd:anyURI ;
    dcat:theme legcons:Section .

C2004A04997:147 a legcons:Item,
        C2004A04997:Item,
        owl:Class,
        dcat:Resource ;
    rdfs:label "Item - I147 Notes"@en-AU ;
    dct:isPartOf C2004A04997:103 ;
    rdfs:comment "Notes - Abrievated Graph Key: I147"@en-AU ;
    rdfs:subClassOf C2004A04997: ;
    skos:definition "Notes"@en-AU ;
    skos:narrower C2004A04997:103 ;
    skos:prefLabel "Item I147"@en-AU ;
    dcat:accessURL <https://www.legislation.gov.au/C2004A04997/2024-07-01/2024-07-01/text/1/epub/OEBPS/document_2/document_2.html#_Toc171750973> ;
    dcat:landingPage "https://www.legislation.gov.au/C2004A04997/2024-07-01/2024-07-01/text/1/epub/OEBPS/document_2/document_2.html#_Toc171750973"^^xsd:anyURI ;
    dcat:theme legcons:Item .

C2004A04997:148 a legcons:Chapter,
        C2004A04997:Chapter,
        owl:Class,
        dcat:Resource ;
    rdfs:label "Chapter - C148 Chapter 28 Inorganic chemicals organic or inorganic compounds of precious metals of rare earth metals of radioactive elements or of isotopes"@en-AU ;
    dct:isPartOf C2004A04997:103 ;
    rdfs:comment "Chapter 28 Inorganic chemicals organic or inorganic compounds of precious metals of rare earth metals of radioactive elements or of isotopes - Abrievated Graph Key: C148"@en-AU ;
    rdfs:subClassOf C2004A04997: ;
    skos:definition "Chapter 28 Inorganic chemicals organic or inorganic compounds of precious metals of rare earth metals of radioactive elements or of isotopes"@en-AU ;
    skos:narrower C2004A04997:103 ;
    skos:prefLabel "Chapter C148"@en-AU ;
    dcat:accessURL <https://www.legislation.gov.au/C2004A04997/2024-07-01/2024-07-01/text/1/epub/OEBPS/document_2/document_2.html#_Toc171750974> ;
    dcat:landingPage "https://www.legislation.gov.au/C2004A04997/2024-07-01/2024-07-01/text/1/epub/OEBPS/document_2/document_2.html#_Toc171750974"^^xsd:anyURI ;
    dcat:theme legcons:Chapter .

C2004A04997:149 a legcons:Item,
        C2004A04997:Item,
        owl:Class,
        dcat:Resource ;
    rdfs:label "Item - I149 Notes"@en-AU ;
    dct:isPartOf C2004A04997:103 ;
    rdfs:comment "Notes - Abrievated Graph Key: I149"@en-AU ;
    rdfs:subClassOf C2004A04997: ;
    skos:definition "Notes"@en-AU ;
    skos:narrower C2004A04997:103 ;
    skos:prefLabel "Item I149"@en-AU ;
    dcat:accessURL <https://www.legislation.gov.au/C2004A04997/2024-07-01/2024-07-01/text/1/epub/OEBPS/document_2/document_2.html#_Toc171750975> ;
    dcat:landingPage "https://www.legislation.gov.au/C2004A04997/2024-07-01/2024-07-01/text/1/epub/OEBPS/document_2/document_2.html#_Toc171750975"^^xsd:anyURI ;
    dcat:theme legcons:Item .

C2004A04997:15 a legcons:Item,
        C2004A04997:Item,
        owl:Class,
        dcat:Resource ;
    rdfs:label "Item - I15 12  Classes of countries and places in relation to which special rates apply"@en-AU ;
    dct:isPartOf C2004A04997:2 ;
    rdfs:comment "12  Classes of countries and places in relation to which special rates apply - Abrievated Graph Key: I15"@en-AU ;
    rdfs:subClassOf C2004A04997: ;
    skos:definition "12  Classes of countries and places in relation to which special rates apply"@en-AU ;
    skos:narrower C2004A04997:2 ;
    skos:prefLabel "Item I15"@en-AU ;
    dcat:accessURL <https://www.legislation.gov.au/C2004A04997/2024-07-01/2024-07-01/text/1/epub/OEBPS/document_1/document_1.html#_Toc172806515> ;
    dcat:landingPage "https://www.legislation.gov.au/C2004A04997/2024-07-01/2024-07-01/text/1/epub/OEBPS/document_1/document_1.html#_Toc172806515"^^xsd:anyURI ;
    dcat:theme legcons:Item .

C2004A04997:150 a legcons:Item,
        C2004A04997:Item,
        owl:Class,
        dcat:Resource ;
    rdfs:label "Item - I150 Subheading Note"@en-AU ;
    dct:isPartOf C2004A04997:103 ;
    rdfs:comment "Subheading Note - Abrievated Graph Key: I150"@en-AU ;
    rdfs:subClassOf C2004A04997: ;
    skos:definition "Subheading Note"@en-AU ;
    skos:narrower C2004A04997:103 ;
    skos:prefLabel "Item I150"@en-AU ;
    dcat:accessURL <https://www.legislation.gov.au/C2004A04997/2024-07-01/2024-07-01/text/1/epub/OEBPS/document_2/document_2.html#_Toc171750976> ;
    dcat:landingPage "https://www.legislation.gov.au/C2004A04997/2024-07-01/2024-07-01/text/1/epub/OEBPS/document_2/document_2.html#_Toc171750976"^^xsd:anyURI ;
    dcat:theme legcons:Item .

C2004A04997:151 a legcons:Item,
        C2004A04997:Item,
        owl:Class,
        dcat:Resource ;
    rdfs:label "Item - I151 Additional Note"@en-AU ;
    dct:isPartOf C2004A04997:103 ;
    rdfs:comment "Additional Note - Abrievated Graph Key: I151"@en-AU ;
    rdfs:subClassOf C2004A04997: ;
    skos:definition "Additional Note"@en-AU ;
    skos:narrower C2004A04997:103 ;
    skos:prefLabel "Item I151"@en-AU ;
    dcat:accessURL <https://www.legislation.gov.au/C2004A04997/2024-07-01/2024-07-01/text/1/epub/OEBPS/document_2/document_2.html#_Toc171750977> ;
    dcat:landingPage "https://www.legislation.gov.au/C2004A04997/2024-07-01/2024-07-01/text/1/epub/OEBPS/document_2/document_2.html#_Toc171750977"^^xsd:anyURI ;
    dcat:theme legcons:Item .

C2004A04997:152 a legcons:Item,
        C2004A04997:Item,
        owl:Class,
        dcat:Resource ;
    rdfs:label "Item - I152 Sub Chapter IChemical elements"@en-AU ;
    dct:isPartOf C2004A04997:103 ;
    rdfs:comment "Sub Chapter IChemical elements - Abrievated Graph Key: I152"@en-AU ;
    rdfs:subClassOf C2004A04997: ;
    skos:definition "Sub Chapter IChemical elements"@en-AU ;
    skos:narrower C2004A04997:103 ;
    skos:prefLabel "Item I152"@en-AU ;
    dcat:accessURL <https://www.legislation.gov.au/C2004A04997/2024-07-01/2024-07-01/text/1/epub/OEBPS/document_2/document_2.html#_Toc171750978> ;
    dcat:landingPage "https://www.legislation.gov.au/C2004A04997/2024-07-01/2024-07-01/text/1/epub/OEBPS/document_2/document_2.html#_Toc171750978"^^xsd:anyURI ;
    dcat:theme legcons:Item .

C2004A04997:153 a legcons:Item,
        C2004A04997:Item,
        owl:Class,
        dcat:Resource ;
    rdfs:label "Item - I153 Sub Chapter IIInorganic acids and inorganic oxygen compounds of non metals"@en-AU ;
    dct:isPartOf C2004A04997:103 ;
    rdfs:comment "Sub Chapter IIInorganic acids and inorganic oxygen compounds of non metals - Abrievated Graph Key: I153"@en-AU ;
    rdfs:subClassOf C2004A04997: ;
    skos:definition "Sub Chapter IIInorganic acids and inorganic oxygen compounds of non metals"@en-AU ;
    skos:narrower C2004A04997:103 ;
    skos:prefLabel "Item I153"@en-AU ;
    dcat:accessURL <https://www.legislation.gov.au/C2004A04997/2024-07-01/2024-07-01/text/1/epub/OEBPS/document_2/document_2.html#_Toc171750979> ;
    dcat:landingPage "https://www.legislation.gov.au/C2004A04997/2024-07-01/2024-07-01/text/1/epub/OEBPS/document_2/document_2.html#_Toc171750979"^^xsd:anyURI ;
    dcat:theme legcons:Item .

C2004A04997:154 a legcons:Item,
        C2004A04997:Item,
        owl:Class,
        dcat:Resource ;
    rdfs:label "Item - I154 Sub Chapter IIIHalogen or sulphur compounds of non metals"@en-AU ;
    dct:isPartOf C2004A04997:103 ;
    rdfs:comment "Sub Chapter IIIHalogen or sulphur compounds of non metals - Abrievated Graph Key: I154"@en-AU ;
    rdfs:subClassOf C2004A04997: ;
    skos:definition "Sub Chapter IIIHalogen or sulphur compounds of non metals"@en-AU ;
    skos:narrower C2004A04997:103 ;
    skos:prefLabel "Item I154"@en-AU ;
    dcat:accessURL <https://www.legislation.gov.au/C2004A04997/2024-07-01/2024-07-01/text/1/epub/OEBPS/document_2/document_2.html#_Toc171750980> ;
    dcat:landingPage "https://www.legislation.gov.au/C2004A04997/2024-07-01/2024-07-01/text/1/epub/OEBPS/document_2/document_2.html#_Toc171750980"^^xsd:anyURI ;
    dcat:theme legcons:Item .

C2004A04997:155 a legcons:Item,
        C2004A04997:Item,
        owl:Class,
        dcat:Resource ;
    rdfs:label "Item - I155 Sub Chapter IVInorganic bases and oxides hydroxides and peroxides of metal"@en-AU ;
    dct:isPartOf C2004A04997:103 ;
    rdfs:comment "Sub Chapter IVInorganic bases and oxides hydroxides and peroxides of metal - Abrievated Graph Key: I155"@en-AU ;
    rdfs:subClassOf C2004A04997: ;
    skos:definition "Sub Chapter IVInorganic bases and oxides hydroxides and peroxides of metal"@en-AU ;
    skos:narrower C2004A04997:103 ;
    skos:prefLabel "Item I155"@en-AU ;
    dcat:accessURL <https://www.legislation.gov.au/C2004A04997/2024-07-01/2024-07-01/text/1/epub/OEBPS/document_2/document_2.html#_Toc171750981> ;
    dcat:landingPage "https://www.legislation.gov.au/C2004A04997/2024-07-01/2024-07-01/text/1/epub/OEBPS/document_2/document_2.html#_Toc171750981"^^xsd:anyURI ;
    dcat:theme legcons:Item .

C2004A04997:156 a legcons:Item,
        C2004A04997:Item,
        owl:Class,
        dcat:Resource ;
    rdfs:label "Item - I156 Sub Chapter VSalts and peroxysalts of inorganic acids and metals"@en-AU ;
    dct:isPartOf C2004A04997:103 ;
    rdfs:comment "Sub Chapter VSalts and peroxysalts of inorganic acids and metals - Abrievated Graph Key: I156"@en-AU ;
    rdfs:subClassOf C2004A04997: ;
    skos:definition "Sub Chapter VSalts and peroxysalts of inorganic acids and metals"@en-AU ;
    skos:narrower C2004A04997:103 ;
    skos:prefLabel "Item I156"@en-AU ;
    dcat:accessURL <https://www.legislation.gov.au/C2004A04997/2024-07-01/2024-07-01/text/1/epub/OEBPS/document_2/document_2.html#_Toc171750982> ;
    dcat:landingPage "https://www.legislation.gov.au/C2004A04997/2024-07-01/2024-07-01/text/1/epub/OEBPS/document_2/document_2.html#_Toc171750982"^^xsd:anyURI ;
    dcat:theme legcons:Item .

C2004A04997:157 a legcons:Item,
        C2004A04997:Item,
        owl:Class,
        dcat:Resource ;
    rdfs:label "Item - I157 Sub Chapter VIMiscellaneous"@en-AU ;
    dct:isPartOf C2004A04997:103 ;
    rdfs:comment "Sub Chapter VIMiscellaneous - Abrievated Graph Key: I157"@en-AU ;
    rdfs:subClassOf C2004A04997: ;
    skos:definition "Sub Chapter VIMiscellaneous"@en-AU ;
    skos:narrower C2004A04997:103 ;
    skos:prefLabel "Item I157"@en-AU ;
    dcat:accessURL <https://www.legislation.gov.au/C2004A04997/2024-07-01/2024-07-01/text/1/epub/OEBPS/document_2/document_2.html#_Toc171750983> ;
    dcat:landingPage "https://www.legislation.gov.au/C2004A04997/2024-07-01/2024-07-01/text/1/epub/OEBPS/document_2/document_2.html#_Toc171750983"^^xsd:anyURI ;
    dcat:theme legcons:Item .

C2004A04997:158 a legcons:Chapter,
        C2004A04997:Chapter,
        owl:Class,
        dcat:Resource ;
    rdfs:label "Chapter - C158 Chapter 29 Organic chemicals"@en-AU ;
    dct:isPartOf C2004A04997:103 ;
    rdfs:comment "Chapter 29 Organic chemicals - Abrievated Graph Key: C158"@en-AU ;
    rdfs:subClassOf C2004A04997: ;
    skos:definition "Chapter 29 Organic chemicals"@en-AU ;
    skos:narrower C2004A04997:103 ;
    skos:prefLabel "Chapter C158"@en-AU ;
    dcat:accessURL <https://www.legislation.gov.au/C2004A04997/2024-07-01/2024-07-01/text/1/epub/OEBPS/document_2/document_2.html#_Toc171750984> ;
    dcat:landingPage "https://www.legislation.gov.au/C2004A04997/2024-07-01/2024-07-01/text/1/epub/OEBPS/document_2/document_2.html#_Toc171750984"^^xsd:anyURI ;
    dcat:theme legcons:Chapter .

C2004A04997:159 a legcons:Item,
        C2004A04997:Item,
        owl:Class,
        dcat:Resource ;
    rdfs:label "Item - I159 Notes"@en-AU ;
    dct:isPartOf C2004A04997:103 ;
    rdfs:comment "Notes - Abrievated Graph Key: I159"@en-AU ;
    rdfs:subClassOf C2004A04997: ;
    skos:definition "Notes"@en-AU ;
    skos:narrower C2004A04997:103 ;
    skos:prefLabel "Item I159"@en-AU ;
    dcat:accessURL <https://www.legislation.gov.au/C2004A04997/2024-07-01/2024-07-01/text/1/epub/OEBPS/document_2/document_2.html#_Toc171750985> ;
    dcat:landingPage "https://www.legislation.gov.au/C2004A04997/2024-07-01/2024-07-01/text/1/epub/OEBPS/document_2/document_2.html#_Toc171750985"^^xsd:anyURI ;
    dcat:theme legcons:Item .

C2004A04997:16 a legcons:Item,
        C2004A04997:Item,
        owl:Class,
        dcat:Resource ;
    rdfs:label "Item - I16 13  When goods are the produce or manufacture of a particular country or place"@en-AU ;
    dct:isPartOf C2004A04997:2 ;
    rdfs:comment "13  When goods are the produce or manufacture of a particular country or place - Abrievated Graph Key: I16"@en-AU ;
    rdfs:subClassOf C2004A04997: ;
    skos:definition "13  When goods are the produce or manufacture of a particular country or place"@en-AU ;
    skos:narrower C2004A04997:2 ;
    skos:prefLabel "Item I16"@en-AU ;
    dcat:accessURL <https://www.legislation.gov.au/C2004A04997/2024-07-01/2024-07-01/text/1/epub/OEBPS/document_1/document_1.html#_Toc172806516> ;
    dcat:landingPage "https://www.legislation.gov.au/C2004A04997/2024-07-01/2024-07-01/text/1/epub/OEBPS/document_1/document_1.html#_Toc172806516"^^xsd:anyURI ;
    dcat:theme legcons:Item .

C2004A04997:160 a legcons:Item,
        C2004A04997:Item,
        owl:Class,
        dcat:Resource ;
    rdfs:label "Item - I160 Subheading Notes"@en-AU ;
    dct:isPartOf C2004A04997:103 ;
    rdfs:comment "Subheading Notes - Abrievated Graph Key: I160"@en-AU ;
    rdfs:subClassOf C2004A04997: ;
    skos:definition "Subheading Notes"@en-AU ;
    skos:narrower C2004A04997:103 ;
    skos:prefLabel "Item I160"@en-AU ;
    dcat:accessURL <https://www.legislation.gov.au/C2004A04997/2024-07-01/2024-07-01/text/1/epub/OEBPS/document_2/document_2.html#_Toc171750986> ;
    dcat:landingPage "https://www.legislation.gov.au/C2004A04997/2024-07-01/2024-07-01/text/1/epub/OEBPS/document_2/document_2.html#_Toc171750986"^^xsd:anyURI ;
    dcat:theme legcons:Item .

C2004A04997:161 a legcons:Item,
        C2004A04997:Item,
        owl:Class,
        dcat:Resource ;
    rdfs:label "Item - I161 Additional Note"@en-AU ;
    dct:isPartOf C2004A04997:103 ;
    rdfs:comment "Additional Note - Abrievated Graph Key: I161"@en-AU ;
    rdfs:subClassOf C2004A04997: ;
    skos:definition "Additional Note"@en-AU ;
    skos:narrower C2004A04997:103 ;
    skos:prefLabel "Item I161"@en-AU ;
    dcat:accessURL <https://www.legislation.gov.au/C2004A04997/2024-07-01/2024-07-01/text/1/epub/OEBPS/document_2/document_2.html#_Toc171750987> ;
    dcat:landingPage "https://www.legislation.gov.au/C2004A04997/2024-07-01/2024-07-01/text/1/epub/OEBPS/document_2/document_2.html#_Toc171750987"^^xsd:anyURI ;
    dcat:theme legcons:Item .

C2004A04997:162 a legcons:Item,
        C2004A04997:Item,
        owl:Class,
        dcat:Resource ;
    rdfs:label "Item - I162 Sub Chapter IHydrocarbons and their halogenated sulphonated nitrated or nitrosated derivatives"@en-AU ;
    dct:isPartOf C2004A04997:103 ;
    rdfs:comment "Sub Chapter IHydrocarbons and their halogenated sulphonated nitrated or nitrosated derivatives - Abrievated Graph Key: I162"@en-AU ;
    rdfs:subClassOf C2004A04997: ;
    skos:definition "Sub Chapter IHydrocarbons and their halogenated sulphonated nitrated or nitrosated derivatives"@en-AU ;
    skos:narrower C2004A04997:103 ;
    skos:prefLabel "Item I162"@en-AU ;
    dcat:accessURL <https://www.legislation.gov.au/C2004A04997/2024-07-01/2024-07-01/text/1/epub/OEBPS/document_2/document_2.html#_Toc171750988> ;
    dcat:landingPage "https://www.legislation.gov.au/C2004A04997/2024-07-01/2024-07-01/text/1/epub/OEBPS/document_2/document_2.html#_Toc171750988"^^xsd:anyURI ;
    dcat:theme legcons:Item .

C2004A04997:163 a legcons:Item,
        C2004A04997:Item,
        owl:Class,
        dcat:Resource ;
    rdfs:label "Item - I163 Sub Chapter IIAlcohols and their halogenated sulphonated nitrated or nitrosated derivatives"@en-AU ;
    dct:isPartOf C2004A04997:103 ;
    rdfs:comment "Sub Chapter IIAlcohols and their halogenated sulphonated nitrated or nitrosated derivatives - Abrievated Graph Key: I163"@en-AU ;
    rdfs:subClassOf C2004A04997: ;
    skos:definition "Sub Chapter IIAlcohols and their halogenated sulphonated nitrated or nitrosated derivatives"@en-AU ;
    skos:narrower C2004A04997:103 ;
    skos:prefLabel "Item I163"@en-AU ;
    dcat:accessURL <https://www.legislation.gov.au/C2004A04997/2024-07-01/2024-07-01/text/1/epub/OEBPS/document_2/document_2.html#_Toc171750989> ;
    dcat:landingPage "https://www.legislation.gov.au/C2004A04997/2024-07-01/2024-07-01/text/1/epub/OEBPS/document_2/document_2.html#_Toc171750989"^^xsd:anyURI ;
    dcat:theme legcons:Item .

C2004A04997:164 a legcons:Item,
        C2004A04997:Item,
        owl:Class,
        dcat:Resource ;
    rdfs:label "Item - I164 Sub Chapter IIIPhenols phenol alcohols and their halogenated sulphonated nitrated or nitrosated derivatives"@en-AU ;
    dct:isPartOf C2004A04997:103 ;
    rdfs:comment "Sub Chapter IIIPhenols phenol alcohols and their halogenated sulphonated nitrated or nitrosated derivatives - Abrievated Graph Key: I164"@en-AU ;
    rdfs:subClassOf C2004A04997: ;
    skos:definition "Sub Chapter IIIPhenols phenol alcohols and their halogenated sulphonated nitrated or nitrosated derivatives"@en-AU ;
    skos:narrower C2004A04997:103 ;
    skos:prefLabel "Item I164"@en-AU ;
    dcat:accessURL <https://www.legislation.gov.au/C2004A04997/2024-07-01/2024-07-01/text/1/epub/OEBPS/document_2/document_2.html#_Toc171750990> ;
    dcat:landingPage "https://www.legislation.gov.au/C2004A04997/2024-07-01/2024-07-01/text/1/epub/OEBPS/document_2/document_2.html#_Toc171750990"^^xsd:anyURI ;
    dcat:theme legcons:Item .

C2004A04997:165 a legcons:Item,
        C2004A04997:Item,
        owl:Class,
        dcat:Resource ;
    rdfs:label "Item - I165 Sub Chapter IVEthers alcohol peroxides ether peroxides acetal and hemiacetal peroxides ketone peroxides epoxides with a three membered ring acetals and hemiacetals and their halogenated sulphonated nitrated or nitrosated derivatives"@en-AU ;
    dct:isPartOf C2004A04997:103 ;
    rdfs:comment "Sub Chapter IVEthers alcohol peroxides ether peroxides acetal and hemiacetal peroxides ketone peroxides epoxides with a three membered ring acetals and hemiacetals and their halogenated sulphonated nitrated or nitrosated derivatives - Abrievated Graph Key: I165"@en-AU ;
    rdfs:subClassOf C2004A04997: ;
    skos:definition "Sub Chapter IVEthers alcohol peroxides ether peroxides acetal and hemiacetal peroxides ketone peroxides epoxides with a three membered ring acetals and hemiacetals and their halogenated sulphonated nitrated or nitrosated derivatives"@en-AU ;
    skos:narrower C2004A04997:103 ;
    skos:prefLabel "Item I165"@en-AU ;
    dcat:accessURL <https://www.legislation.gov.au/C2004A04997/2024-07-01/2024-07-01/text/1/epub/OEBPS/document_2/document_2.html#_Toc171750991> ;
    dcat:landingPage "https://www.legislation.gov.au/C2004A04997/2024-07-01/2024-07-01/text/1/epub/OEBPS/document_2/document_2.html#_Toc171750991"^^xsd:anyURI ;
    dcat:theme legcons:Item .

C2004A04997:166 a legcons:Item,
        C2004A04997:Item,
        owl:Class,
        dcat:Resource ;
    rdfs:label "Item - I166 Sub Chapter VAldehyde function compounds"@en-AU ;
    dct:isPartOf C2004A04997:103 ;
    rdfs:comment "Sub Chapter VAldehyde function compounds - Abrievated Graph Key: I166"@en-AU ;
    rdfs:subClassOf C2004A04997: ;
    skos:definition "Sub Chapter VAldehyde function compounds"@en-AU ;
    skos:narrower C2004A04997:103 ;
    skos:prefLabel "Item I166"@en-AU ;
    dcat:accessURL <https://www.legislation.gov.au/C2004A04997/2024-07-01/2024-07-01/text/1/epub/OEBPS/document_2/document_2.html#_Toc171750992> ;
    dcat:landingPage "https://www.legislation.gov.au/C2004A04997/2024-07-01/2024-07-01/text/1/epub/OEBPS/document_2/document_2.html#_Toc171750992"^^xsd:anyURI ;
    dcat:theme legcons:Item .

C2004A04997:167 a legcons:Item,
        C2004A04997:Item,
        owl:Class,
        dcat:Resource ;
    rdfs:label "Item - I167 Sub Chapter VIKetone function compounds and quinone function compounds"@en-AU ;
    dct:isPartOf C2004A04997:103 ;
    rdfs:comment "Sub Chapter VIKetone function compounds and quinone function compounds - Abrievated Graph Key: I167"@en-AU ;
    rdfs:subClassOf C2004A04997: ;
    skos:definition "Sub Chapter VIKetone function compounds and quinone function compounds"@en-AU ;
    skos:narrower C2004A04997:103 ;
    skos:prefLabel "Item I167"@en-AU ;
    dcat:accessURL <https://www.legislation.gov.au/C2004A04997/2024-07-01/2024-07-01/text/1/epub/OEBPS/document_2/document_2.html#_Toc171750993> ;
    dcat:landingPage "https://www.legislation.gov.au/C2004A04997/2024-07-01/2024-07-01/text/1/epub/OEBPS/document_2/document_2.html#_Toc171750993"^^xsd:anyURI ;
    dcat:theme legcons:Item .

C2004A04997:168 a legcons:Item,
        C2004A04997:Item,
        owl:Class,
        dcat:Resource ;
    rdfs:label "Item - I168 Sub Chapter VIICarboxylic acids and their anhydrides halides peroxides and peroxyacids and their halogenated sulphonated nitrated or nitrosated derivatives"@en-AU ;
    dct:isPartOf C2004A04997:103 ;
    rdfs:comment "Sub Chapter VIICarboxylic acids and their anhydrides halides peroxides and peroxyacids and their halogenated sulphonated nitrated or nitrosated derivatives - Abrievated Graph Key: I168"@en-AU ;
    rdfs:subClassOf C2004A04997: ;
    skos:definition "Sub Chapter VIICarboxylic acids and their anhydrides halides peroxides and peroxyacids and their halogenated sulphonated nitrated or nitrosated derivatives"@en-AU ;
    skos:narrower C2004A04997:103 ;
    skos:prefLabel "Item I168"@en-AU ;
    dcat:accessURL <https://www.legislation.gov.au/C2004A04997/2024-07-01/2024-07-01/text/1/epub/OEBPS/document_2/document_2.html#_Toc171750994> ;
    dcat:landingPage "https://www.legislation.gov.au/C2004A04997/2024-07-01/2024-07-01/text/1/epub/OEBPS/document_2/document_2.html#_Toc171750994"^^xsd:anyURI ;
    dcat:theme legcons:Item .

C2004A04997:169 a legcons:Item,
        C2004A04997:Item,
        owl:Class,
        dcat:Resource ;
    rdfs:label "Item - I169 Sub Chapter VIIIEsters of inorganic acids of non metals and their salts and their halogenated sulphonated nitrated or nitrosated derivatives"@en-AU ;
    dct:isPartOf C2004A04997:103 ;
    rdfs:comment "Sub Chapter VIIIEsters of inorganic acids of non metals and their salts and their halogenated sulphonated nitrated or nitrosated derivatives - Abrievated Graph Key: I169"@en-AU ;
    rdfs:subClassOf C2004A04997: ;
    skos:definition "Sub Chapter VIIIEsters of inorganic acids of non metals and their salts and their halogenated sulphonated nitrated or nitrosated derivatives"@en-AU ;
    skos:narrower C2004A04997:103 ;
    skos:prefLabel "Item I169"@en-AU ;
    dcat:accessURL <https://www.legislation.gov.au/C2004A04997/2024-07-01/2024-07-01/text/1/epub/OEBPS/document_2/document_2.html#_Toc171750995> ;
    dcat:landingPage "https://www.legislation.gov.au/C2004A04997/2024-07-01/2024-07-01/text/1/epub/OEBPS/document_2/document_2.html#_Toc171750995"^^xsd:anyURI ;
    dcat:theme legcons:Item .

C2004A04997:17 a legcons:Item,
        C2004A04997:Item,
        owl:Class,
        dcat:Resource ;
    rdfs:label "Item - I17 13 AA  When goods are Singaporean originating goods"@en-AU ;
    dct:isPartOf C2004A04997:2 ;
    rdfs:comment "13 AA  When goods are Singaporean originating goods - Abrievated Graph Key: I17"@en-AU ;
    rdfs:subClassOf C2004A04997: ;
    skos:definition "13 AA  When goods are Singaporean originating goods"@en-AU ;
    skos:narrower C2004A04997:2 ;
    skos:prefLabel "Item I17"@en-AU ;
    dcat:accessURL <https://www.legislation.gov.au/C2004A04997/2024-07-01/2024-07-01/text/1/epub/OEBPS/document_1/document_1.html#_Toc172806517> ;
    dcat:landingPage "https://www.legislation.gov.au/C2004A04997/2024-07-01/2024-07-01/text/1/epub/OEBPS/document_1/document_1.html#_Toc172806517"^^xsd:anyURI ;
    dcat:theme legcons:Item .

C2004A04997:170 a legcons:Item,
        C2004A04997:Item,
        owl:Class,
        dcat:Resource ;
    rdfs:label "Item - I170 Sub Chapter IXNitrogen function compounds"@en-AU ;
    dct:isPartOf C2004A04997:103 ;
    rdfs:comment "Sub Chapter IXNitrogen function compounds - Abrievated Graph Key: I170"@en-AU ;
    rdfs:subClassOf C2004A04997: ;
    skos:definition "Sub Chapter IXNitrogen function compounds"@en-AU ;
    skos:narrower C2004A04997:103 ;
    skos:prefLabel "Item I170"@en-AU ;
    dcat:accessURL <https://www.legislation.gov.au/C2004A04997/2024-07-01/2024-07-01/text/1/epub/OEBPS/document_2/document_2.html#_Toc171750996> ;
    dcat:landingPage "https://www.legislation.gov.au/C2004A04997/2024-07-01/2024-07-01/text/1/epub/OEBPS/document_2/document_2.html#_Toc171750996"^^xsd:anyURI ;
    dcat:theme legcons:Item .

C2004A04997:171 a legcons:Item,
        C2004A04997:Item,
        owl:Class,
        dcat:Resource ;
    rdfs:label "Item - I171 Sub Chapter XOrgano inorganic compounds heterocyclic compounds nucleic acids and their salts and sulphonamides"@en-AU ;
    dct:isPartOf C2004A04997:103 ;
    rdfs:comment "Sub Chapter XOrgano inorganic compounds heterocyclic compounds nucleic acids and their salts and sulphonamides - Abrievated Graph Key: I171"@en-AU ;
    rdfs:subClassOf C2004A04997: ;
    skos:definition "Sub Chapter XOrgano inorganic compounds heterocyclic compounds nucleic acids and their salts and sulphonamides"@en-AU ;
    skos:narrower C2004A04997:103 ;
    skos:prefLabel "Item I171"@en-AU ;
    dcat:accessURL <https://www.legislation.gov.au/C2004A04997/2024-07-01/2024-07-01/text/1/epub/OEBPS/document_2/document_2.html#_Toc171750997> ;
    dcat:landingPage "https://www.legislation.gov.au/C2004A04997/2024-07-01/2024-07-01/text/1/epub/OEBPS/document_2/document_2.html#_Toc171750997"^^xsd:anyURI ;
    dcat:theme legcons:Item .

C2004A04997:172 a legcons:Item,
        C2004A04997:Item,
        owl:Class,
        dcat:Resource ;
    rdfs:label "Item - I172 Sub Chapter XIProvitamins vitamins and hormones"@en-AU ;
    dct:isPartOf C2004A04997:103 ;
    rdfs:comment "Sub Chapter XIProvitamins vitamins and hormones - Abrievated Graph Key: I172"@en-AU ;
    rdfs:subClassOf C2004A04997: ;
    skos:definition "Sub Chapter XIProvitamins vitamins and hormones"@en-AU ;
    skos:narrower C2004A04997:103 ;
    skos:prefLabel "Item I172"@en-AU ;
    dcat:accessURL <https://www.legislation.gov.au/C2004A04997/2024-07-01/2024-07-01/text/1/epub/OEBPS/document_2/document_2.html#_Toc171750998> ;
    dcat:landingPage "https://www.legislation.gov.au/C2004A04997/2024-07-01/2024-07-01/text/1/epub/OEBPS/document_2/document_2.html#_Toc171750998"^^xsd:anyURI ;
    dcat:theme legcons:Item .

C2004A04997:173 a legcons:Item,
        C2004A04997:Item,
        owl:Class,
        dcat:Resource ;
    rdfs:label "Item - I173 Sub Chapter XIIGlycosides and alkaloids natural or reproduced by synthesis and their salts ethers esters and other derivatives"@en-AU ;
    dct:isPartOf C2004A04997:103 ;
    rdfs:comment "Sub Chapter XIIGlycosides and alkaloids natural or reproduced by synthesis and their salts ethers esters and other derivatives - Abrievated Graph Key: I173"@en-AU ;
    rdfs:subClassOf C2004A04997: ;
    skos:definition "Sub Chapter XIIGlycosides and alkaloids natural or reproduced by synthesis and their salts ethers esters and other derivatives"@en-AU ;
    skos:narrower C2004A04997:103 ;
    skos:prefLabel "Item I173"@en-AU ;
    dcat:accessURL <https://www.legislation.gov.au/C2004A04997/2024-07-01/2024-07-01/text/1/epub/OEBPS/document_2/document_2.html#_Toc171750999> ;
    dcat:landingPage "https://www.legislation.gov.au/C2004A04997/2024-07-01/2024-07-01/text/1/epub/OEBPS/document_2/document_2.html#_Toc171750999"^^xsd:anyURI ;
    dcat:theme legcons:Item .

C2004A04997:174 a legcons:Item,
        C2004A04997:Item,
        owl:Class,
        dcat:Resource ;
    rdfs:label "Item - I174 Sub Chapter XIIIOther organic compounds"@en-AU ;
    dct:isPartOf C2004A04997:103 ;
    rdfs:comment "Sub Chapter XIIIOther organic compounds - Abrievated Graph Key: I174"@en-AU ;
    rdfs:subClassOf C2004A04997: ;
    skos:definition "Sub Chapter XIIIOther organic compounds"@en-AU ;
    skos:narrower C2004A04997:103 ;
    skos:prefLabel "Item I174"@en-AU ;
    dcat:accessURL <https://www.legislation.gov.au/C2004A04997/2024-07-01/2024-07-01/text/1/epub/OEBPS/document_2/document_2.html#_Toc171751000> ;
    dcat:landingPage "https://www.legislation.gov.au/C2004A04997/2024-07-01/2024-07-01/text/1/epub/OEBPS/document_2/document_2.html#_Toc171751000"^^xsd:anyURI ;
    dcat:theme legcons:Item .

C2004A04997:175 a legcons:Chapter,
        C2004A04997:Chapter,
        owl:Class,
        dcat:Resource ;
    rdfs:label "Chapter - C175 Chapter 30 Pharmaceutical products"@en-AU ;
    dct:isPartOf C2004A04997:103 ;
    rdfs:comment "Chapter 30 Pharmaceutical products - Abrievated Graph Key: C175"@en-AU ;
    rdfs:subClassOf C2004A04997: ;
    skos:definition "Chapter 30 Pharmaceutical products"@en-AU ;
    skos:narrower C2004A04997:103 ;
    skos:prefLabel "Chapter C175"@en-AU ;
    dcat:accessURL <https://www.legislation.gov.au/C2004A04997/2024-07-01/2024-07-01/text/1/epub/OEBPS/document_2/document_2.html#_Toc171751001> ;
    dcat:landingPage "https://www.legislation.gov.au/C2004A04997/2024-07-01/2024-07-01/text/1/epub/OEBPS/document_2/document_2.html#_Toc171751001"^^xsd:anyURI ;
    dcat:theme legcons:Chapter .

C2004A04997:176 a legcons:Item,
        C2004A04997:Item,
        owl:Class,
        dcat:Resource ;
    rdfs:label "Item - I176 Notes"@en-AU ;
    dct:isPartOf C2004A04997:103 ;
    rdfs:comment "Notes - Abrievated Graph Key: I176"@en-AU ;
    rdfs:subClassOf C2004A04997: ;
    skos:definition "Notes"@en-AU ;
    skos:narrower C2004A04997:103 ;
    skos:prefLabel "Item I176"@en-AU ;
    dcat:accessURL <https://www.legislation.gov.au/C2004A04997/2024-07-01/2024-07-01/text/1/epub/OEBPS/document_2/document_2.html#_Toc171751002> ;
    dcat:landingPage "https://www.legislation.gov.au/C2004A04997/2024-07-01/2024-07-01/text/1/epub/OEBPS/document_2/document_2.html#_Toc171751002"^^xsd:anyURI ;
    dcat:theme legcons:Item .

C2004A04997:177 a legcons:Item,
        C2004A04997:Item,
        owl:Class,
        dcat:Resource ;
    rdfs:label "Item - I177 Subheading Notes"@en-AU ;
    dct:isPartOf C2004A04997:103 ;
    rdfs:comment "Subheading Notes - Abrievated Graph Key: I177"@en-AU ;
    rdfs:subClassOf C2004A04997: ;
    skos:definition "Subheading Notes"@en-AU ;
    skos:narrower C2004A04997:103 ;
    skos:prefLabel "Item I177"@en-AU ;
    dcat:accessURL <https://www.legislation.gov.au/C2004A04997/2024-07-01/2024-07-01/text/1/epub/OEBPS/document_2/document_2.html#_Toc171751003> ;
    dcat:landingPage "https://www.legislation.gov.au/C2004A04997/2024-07-01/2024-07-01/text/1/epub/OEBPS/document_2/document_2.html#_Toc171751003"^^xsd:anyURI ;
    dcat:theme legcons:Item .

C2004A04997:178 a legcons:Item,
        C2004A04997:Item,
        owl:Class,
        dcat:Resource ;
    rdfs:label "Item - I178 Additional Notes"@en-AU ;
    dct:isPartOf C2004A04997:103 ;
    rdfs:comment "Additional Notes - Abrievated Graph Key: I178"@en-AU ;
    rdfs:subClassOf C2004A04997: ;
    skos:definition "Additional Notes"@en-AU ;
    skos:narrower C2004A04997:103 ;
    skos:prefLabel "Item I178"@en-AU ;
    dcat:accessURL <https://www.legislation.gov.au/C2004A04997/2024-07-01/2024-07-01/text/1/epub/OEBPS/document_2/document_2.html#_Toc171751004> ;
    dcat:landingPage "https://www.legislation.gov.au/C2004A04997/2024-07-01/2024-07-01/text/1/epub/OEBPS/document_2/document_2.html#_Toc171751004"^^xsd:anyURI ;
    dcat:theme legcons:Item .

C2004A04997:179 a legcons:Chapter,
        C2004A04997:Chapter,
        owl:Class,
        dcat:Resource ;
    rdfs:label "Chapter - C179 Chapter 31 Fertilisers"@en-AU ;
    dct:isPartOf C2004A04997:103 ;
    rdfs:comment "Chapter 31 Fertilisers - Abrievated Graph Key: C179"@en-AU ;
    rdfs:subClassOf C2004A04997: ;
    skos:definition "Chapter 31 Fertilisers"@en-AU ;
    skos:narrower C2004A04997:103 ;
    skos:prefLabel "Chapter C179"@en-AU ;
    dcat:accessURL <https://www.legislation.gov.au/C2004A04997/2024-07-01/2024-07-01/text/1/epub/OEBPS/document_2/document_2.html#_Toc171751005> ;
    dcat:landingPage "https://www.legislation.gov.au/C2004A04997/2024-07-01/2024-07-01/text/1/epub/OEBPS/document_2/document_2.html#_Toc171751005"^^xsd:anyURI ;
    dcat:theme legcons:Chapter .

C2004A04997:18 a legcons:Item,
        C2004A04997:Item,
        owl:Class,
        dcat:Resource ;
    rdfs:label "Item - I18 13 A  When goods are US originating goods"@en-AU ;
    dct:isPartOf C2004A04997:2 ;
    rdfs:comment "13 A  When goods are US originating goods - Abrievated Graph Key: I18"@en-AU ;
    rdfs:subClassOf C2004A04997: ;
    skos:definition "13 A  When goods are US originating goods"@en-AU ;
    skos:narrower C2004A04997:2 ;
    skos:prefLabel "Item I18"@en-AU ;
    dcat:accessURL <https://www.legislation.gov.au/C2004A04997/2024-07-01/2024-07-01/text/1/epub/OEBPS/document_1/document_1.html#_Toc172806518> ;
    dcat:landingPage "https://www.legislation.gov.au/C2004A04997/2024-07-01/2024-07-01/text/1/epub/OEBPS/document_1/document_1.html#_Toc172806518"^^xsd:anyURI ;
    dcat:theme legcons:Item .

C2004A04997:180 a legcons:Item,
        C2004A04997:Item,
        owl:Class,
        dcat:Resource ;
    rdfs:label "Item - I180 Notes"@en-AU ;
    dct:isPartOf C2004A04997:103 ;
    rdfs:comment "Notes - Abrievated Graph Key: I180"@en-AU ;
    rdfs:subClassOf C2004A04997: ;
    skos:definition "Notes"@en-AU ;
    skos:narrower C2004A04997:103 ;
    skos:prefLabel "Item I180"@en-AU ;
    dcat:accessURL <https://www.legislation.gov.au/C2004A04997/2024-07-01/2024-07-01/text/1/epub/OEBPS/document_2/document_2.html#_Toc171751006> ;
    dcat:landingPage "https://www.legislation.gov.au/C2004A04997/2024-07-01/2024-07-01/text/1/epub/OEBPS/document_2/document_2.html#_Toc171751006"^^xsd:anyURI ;
    dcat:theme legcons:Item .

C2004A04997:181 a legcons:Chapter,
        C2004A04997:Chapter,
        owl:Class,
        dcat:Resource ;
    rdfs:label "Chapter - C181 Chapter 32 Tanning or dyeing extracts tannins and their derivatives dyes pigments and other colouring matter paints and varnishes putty and other mastics inks"@en-AU ;
    dct:isPartOf C2004A04997:103 ;
    rdfs:comment "Chapter 32 Tanning or dyeing extracts tannins and their derivatives dyes pigments and other colouring matter paints and varnishes putty and other mastics inks - Abrievated Graph Key: C181"@en-AU ;
    rdfs:subClassOf C2004A04997: ;
    skos:definition "Chapter 32 Tanning or dyeing extracts tannins and their derivatives dyes pigments and other colouring matter paints and varnishes putty and other mastics inks"@en-AU ;
    skos:narrower C2004A04997:103 ;
    skos:prefLabel "Chapter C181"@en-AU ;
    dcat:accessURL <https://www.legislation.gov.au/C2004A04997/2024-07-01/2024-07-01/text/1/epub/OEBPS/document_2/document_2.html#_Toc171751007> ;
    dcat:landingPage "https://www.legislation.gov.au/C2004A04997/2024-07-01/2024-07-01/text/1/epub/OEBPS/document_2/document_2.html#_Toc171751007"^^xsd:anyURI ;
    dcat:theme legcons:Chapter .

C2004A04997:182 a legcons:Item,
        C2004A04997:Item,
        owl:Class,
        dcat:Resource ;
    rdfs:label "Item - I182 Notes"@en-AU ;
    dct:isPartOf C2004A04997:103 ;
    rdfs:comment "Notes - Abrievated Graph Key: I182"@en-AU ;
    rdfs:subClassOf C2004A04997: ;
    skos:definition "Notes"@en-AU ;
    skos:narrower C2004A04997:103 ;
    skos:prefLabel "Item I182"@en-AU ;
    dcat:accessURL <https://www.legislation.gov.au/C2004A04997/2024-07-01/2024-07-01/text/1/epub/OEBPS/document_2/document_2.html#_Toc171751008> ;
    dcat:landingPage "https://www.legislation.gov.au/C2004A04997/2024-07-01/2024-07-01/text/1/epub/OEBPS/document_2/document_2.html#_Toc171751008"^^xsd:anyURI ;
    dcat:theme legcons:Item .

C2004A04997:183 a legcons:Chapter,
        C2004A04997:Chapter,
        owl:Class,
        dcat:Resource ;
    rdfs:label "Chapter - C183 Chapter 33 Essential oils and resinoids perfumery cosmetic or toilet preparations"@en-AU ;
    dct:isPartOf C2004A04997:103 ;
    rdfs:comment "Chapter 33 Essential oils and resinoids perfumery cosmetic or toilet preparations - Abrievated Graph Key: C183"@en-AU ;
    rdfs:subClassOf C2004A04997: ;
    skos:definition "Chapter 33 Essential oils and resinoids perfumery cosmetic or toilet preparations"@en-AU ;
    skos:narrower C2004A04997:103 ;
    skos:prefLabel "Chapter C183"@en-AU ;
    dcat:accessURL <https://www.legislation.gov.au/C2004A04997/2024-07-01/2024-07-01/text/1/epub/OEBPS/document_2/document_2.html#_Toc171751009> ;
    dcat:landingPage "https://www.legislation.gov.au/C2004A04997/2024-07-01/2024-07-01/text/1/epub/OEBPS/document_2/document_2.html#_Toc171751009"^^xsd:anyURI ;
    dcat:theme legcons:Chapter .

C2004A04997:184 a legcons:Item,
        C2004A04997:Item,
        owl:Class,
        dcat:Resource ;
    rdfs:label "Item - I184 Notes"@en-AU ;
    dct:isPartOf C2004A04997:103 ;
    rdfs:comment "Notes - Abrievated Graph Key: I184"@en-AU ;
    rdfs:subClassOf C2004A04997: ;
    skos:definition "Notes"@en-AU ;
    skos:narrower C2004A04997:103 ;
    skos:prefLabel "Item I184"@en-AU ;
    dcat:accessURL <https://www.legislation.gov.au/C2004A04997/2024-07-01/2024-07-01/text/1/epub/OEBPS/document_2/document_2.html#_Toc171751010> ;
    dcat:landingPage "https://www.legislation.gov.au/C2004A04997/2024-07-01/2024-07-01/text/1/epub/OEBPS/document_2/document_2.html#_Toc171751010"^^xsd:anyURI ;
    dcat:theme legcons:Item .

C2004A04997:185 a legcons:Chapter,
        C2004A04997:Chapter,
        owl:Class,
        dcat:Resource ;
    rdfs:label "Chapter - C185 Chapter 34 Soap organic surface active agents washing preparations lubricating preparations artificial waxes prepared waxes polishing or scouring preparations candles and similar articles modelling pastes dental waxes and dental preparations with a basis of plaster"@en-AU ;
    dct:isPartOf C2004A04997:103 ;
    rdfs:comment "Chapter 34 Soap organic surface active agents washing preparations lubricating preparations artificial waxes prepared waxes polishing or scouring preparations candles and similar articles modelling pastes dental waxes and dental preparations with a basis of plaster - Abrievated Graph Key: C185"@en-AU ;
    rdfs:subClassOf C2004A04997: ;
    skos:definition "Chapter 34 Soap organic surface active agents washing preparations lubricating preparations artificial waxes prepared waxes polishing or scouring preparations candles and similar articles modelling pastes dental waxes and dental preparations with a basis of plaster"@en-AU ;
    skos:narrower C2004A04997:103 ;
    skos:prefLabel "Chapter C185"@en-AU ;
    dcat:accessURL <https://www.legislation.gov.au/C2004A04997/2024-07-01/2024-07-01/text/1/epub/OEBPS/document_2/document_2.html#_Toc171751011> ;
    dcat:landingPage "https://www.legislation.gov.au/C2004A04997/2024-07-01/2024-07-01/text/1/epub/OEBPS/document_2/document_2.html#_Toc171751011"^^xsd:anyURI ;
    dcat:theme legcons:Chapter .

C2004A04997:186 a legcons:Item,
        C2004A04997:Item,
        owl:Class,
        dcat:Resource ;
    rdfs:label "Item - I186 Notes"@en-AU ;
    dct:isPartOf C2004A04997:103 ;
    rdfs:comment "Notes - Abrievated Graph Key: I186"@en-AU ;
    rdfs:subClassOf C2004A04997: ;
    skos:definition "Notes"@en-AU ;
    skos:narrower C2004A04997:103 ;
    skos:prefLabel "Item I186"@en-AU ;
    dcat:accessURL <https://www.legislation.gov.au/C2004A04997/2024-07-01/2024-07-01/text/1/epub/OEBPS/document_2/document_2.html#_Toc171751012> ;
    dcat:landingPage "https://www.legislation.gov.au/C2004A04997/2024-07-01/2024-07-01/text/1/epub/OEBPS/document_2/document_2.html#_Toc171751012"^^xsd:anyURI ;
    dcat:theme legcons:Item .

C2004A04997:187 a legcons:Chapter,
        C2004A04997:Chapter,
        owl:Class,
        dcat:Resource ;
    rdfs:label "Chapter - C187 Chapter 35 Albuminoidal substances modified starches glues enzymes"@en-AU ;
    dct:isPartOf C2004A04997:103 ;
    rdfs:comment "Chapter 35 Albuminoidal substances modified starches glues enzymes - Abrievated Graph Key: C187"@en-AU ;
    rdfs:subClassOf C2004A04997: ;
    skos:definition "Chapter 35 Albuminoidal substances modified starches glues enzymes"@en-AU ;
    skos:narrower C2004A04997:103 ;
    skos:prefLabel "Chapter C187"@en-AU ;
    dcat:accessURL <https://www.legislation.gov.au/C2004A04997/2024-07-01/2024-07-01/text/1/epub/OEBPS/document_2/document_2.html#_Toc171751013> ;
    dcat:landingPage "https://www.legislation.gov.au/C2004A04997/2024-07-01/2024-07-01/text/1/epub/OEBPS/document_2/document_2.html#_Toc171751013"^^xsd:anyURI ;
    dcat:theme legcons:Chapter .

C2004A04997:188 a legcons:Item,
        C2004A04997:Item,
        owl:Class,
        dcat:Resource ;
    rdfs:label "Item - I188 Notes"@en-AU ;
    dct:isPartOf C2004A04997:103 ;
    rdfs:comment "Notes - Abrievated Graph Key: I188"@en-AU ;
    rdfs:subClassOf C2004A04997: ;
    skos:definition "Notes"@en-AU ;
    skos:narrower C2004A04997:103 ;
    skos:prefLabel "Item I188"@en-AU ;
    dcat:accessURL <https://www.legislation.gov.au/C2004A04997/2024-07-01/2024-07-01/text/1/epub/OEBPS/document_2/document_2.html#_Toc171751014> ;
    dcat:landingPage "https://www.legislation.gov.au/C2004A04997/2024-07-01/2024-07-01/text/1/epub/OEBPS/document_2/document_2.html#_Toc171751014"^^xsd:anyURI ;
    dcat:theme legcons:Item .

C2004A04997:189 a legcons:Chapter,
        C2004A04997:Chapter,
        owl:Class,
        dcat:Resource ;
    rdfs:label "Chapter - C189 Chapter 36 Explosives pyrotechnic products matches pyrophoric alloys certain combustible preparations"@en-AU ;
    dct:isPartOf C2004A04997:103 ;
    rdfs:comment "Chapter 36 Explosives pyrotechnic products matches pyrophoric alloys certain combustible preparations - Abrievated Graph Key: C189"@en-AU ;
    rdfs:subClassOf C2004A04997: ;
    skos:definition "Chapter 36 Explosives pyrotechnic products matches pyrophoric alloys certain combustible preparations"@en-AU ;
    skos:narrower C2004A04997:103 ;
    skos:prefLabel "Chapter C189"@en-AU ;
    dcat:accessURL <https://www.legislation.gov.au/C2004A04997/2024-07-01/2024-07-01/text/1/epub/OEBPS/document_2/document_2.html#_Toc171751015> ;
    dcat:landingPage "https://www.legislation.gov.au/C2004A04997/2024-07-01/2024-07-01/text/1/epub/OEBPS/document_2/document_2.html#_Toc171751015"^^xsd:anyURI ;
    dcat:theme legcons:Chapter .

C2004A04997:19 a legcons:Item,
        C2004A04997:Item,
        owl:Class,
        dcat:Resource ;
    rdfs:label "Item - I19 13 B  When goods are Thai originating goods"@en-AU ;
    dct:isPartOf C2004A04997:2 ;
    rdfs:comment "13 B  When goods are Thai originating goods - Abrievated Graph Key: I19"@en-AU ;
    rdfs:subClassOf C2004A04997: ;
    skos:definition "13 B  When goods are Thai originating goods"@en-AU ;
    skos:narrower C2004A04997:2 ;
    skos:prefLabel "Item I19"@en-AU ;
    dcat:accessURL <https://www.legislation.gov.au/C2004A04997/2024-07-01/2024-07-01/text/1/epub/OEBPS/document_1/document_1.html#_Toc172806519> ;
    dcat:landingPage "https://www.legislation.gov.au/C2004A04997/2024-07-01/2024-07-01/text/1/epub/OEBPS/document_1/document_1.html#_Toc172806519"^^xsd:anyURI ;
    dcat:theme legcons:Item .

C2004A04997:190 a legcons:Item,
        C2004A04997:Item,
        owl:Class,
        dcat:Resource ;
    rdfs:label "Item - I190 Notes"@en-AU ;
    dct:isPartOf C2004A04997:103 ;
    rdfs:comment "Notes - Abrievated Graph Key: I190"@en-AU ;
    rdfs:subClassOf C2004A04997: ;
    skos:definition "Notes"@en-AU ;
    skos:narrower C2004A04997:103 ;
    skos:prefLabel "Item I190"@en-AU ;
    dcat:accessURL <https://www.legislation.gov.au/C2004A04997/2024-07-01/2024-07-01/text/1/epub/OEBPS/document_2/document_2.html#_Toc171751016> ;
    dcat:landingPage "https://www.legislation.gov.au/C2004A04997/2024-07-01/2024-07-01/text/1/epub/OEBPS/document_2/document_2.html#_Toc171751016"^^xsd:anyURI ;
    dcat:theme legcons:Item .

C2004A04997:191 a legcons:Chapter,
        C2004A04997:Chapter,
        owl:Class,
        dcat:Resource ;
    rdfs:label "Chapter - C191 Chapter 37 Photographic or cinematographic goods"@en-AU ;
    dct:isPartOf C2004A04997:103 ;
    rdfs:comment "Chapter 37 Photographic or cinematographic goods - Abrievated Graph Key: C191"@en-AU ;
    rdfs:subClassOf C2004A04997: ;
    skos:definition "Chapter 37 Photographic or cinematographic goods"@en-AU ;
    skos:narrower C2004A04997:103 ;
    skos:prefLabel "Chapter C191"@en-AU ;
    dcat:accessURL <https://www.legislation.gov.au/C2004A04997/2024-07-01/2024-07-01/text/1/epub/OEBPS/document_2/document_2.html#_Toc171751017> ;
    dcat:landingPage "https://www.legislation.gov.au/C2004A04997/2024-07-01/2024-07-01/text/1/epub/OEBPS/document_2/document_2.html#_Toc171751017"^^xsd:anyURI ;
    dcat:theme legcons:Chapter .

C2004A04997:192 a legcons:Item,
        C2004A04997:Item,
        owl:Class,
        dcat:Resource ;
    rdfs:label "Item - I192 Notes"@en-AU ;
    dct:isPartOf C2004A04997:103 ;
    rdfs:comment "Notes - Abrievated Graph Key: I192"@en-AU ;
    rdfs:subClassOf C2004A04997: ;
    skos:definition "Notes"@en-AU ;
    skos:narrower C2004A04997:103 ;
    skos:prefLabel "Item I192"@en-AU ;
    dcat:accessURL <https://www.legislation.gov.au/C2004A04997/2024-07-01/2024-07-01/text/1/epub/OEBPS/document_2/document_2.html#_Toc171751018> ;
    dcat:landingPage "https://www.legislation.gov.au/C2004A04997/2024-07-01/2024-07-01/text/1/epub/OEBPS/document_2/document_2.html#_Toc171751018"^^xsd:anyURI ;
    dcat:theme legcons:Item .

C2004A04997:193 a legcons:Chapter,
        C2004A04997:Chapter,
        owl:Class,
        dcat:Resource ;
    rdfs:label "Chapter - C193 Chapter 38 Miscellaneous chemical products"@en-AU ;
    dct:isPartOf C2004A04997:103 ;
    rdfs:comment "Chapter 38 Miscellaneous chemical products - Abrievated Graph Key: C193"@en-AU ;
    rdfs:subClassOf C2004A04997: ;
    skos:definition "Chapter 38 Miscellaneous chemical products"@en-AU ;
    skos:narrower C2004A04997:103 ;
    skos:prefLabel "Chapter C193"@en-AU ;
    dcat:accessURL <https://www.legislation.gov.au/C2004A04997/2024-07-01/2024-07-01/text/1/epub/OEBPS/document_2/document_2.html#_Toc171751019> ;
    dcat:landingPage "https://www.legislation.gov.au/C2004A04997/2024-07-01/2024-07-01/text/1/epub/OEBPS/document_2/document_2.html#_Toc171751019"^^xsd:anyURI ;
    dcat:theme legcons:Chapter .

C2004A04997:194 a legcons:Item,
        C2004A04997:Item,
        owl:Class,
        dcat:Resource ;
    rdfs:label "Item - I194 Notes"@en-AU ;
    dct:isPartOf C2004A04997:103 ;
    rdfs:comment "Notes - Abrievated Graph Key: I194"@en-AU ;
    rdfs:subClassOf C2004A04997: ;
    skos:definition "Notes"@en-AU ;
    skos:narrower C2004A04997:103 ;
    skos:prefLabel "Item I194"@en-AU ;
    dcat:accessURL <https://www.legislation.gov.au/C2004A04997/2024-07-01/2024-07-01/text/1/epub/OEBPS/document_2/document_2.html#_Toc171751020> ;
    dcat:landingPage "https://www.legislation.gov.au/C2004A04997/2024-07-01/2024-07-01/text/1/epub/OEBPS/document_2/document_2.html#_Toc171751020"^^xsd:anyURI ;
    dcat:theme legcons:Item .

C2004A04997:195 a legcons:Item,
        C2004A04997:Item,
        owl:Class,
        dcat:Resource ;
    rdfs:label "Item - I195 Subheading Notes"@en-AU ;
    dct:isPartOf C2004A04997:103 ;
    rdfs:comment "Subheading Notes - Abrievated Graph Key: I195"@en-AU ;
    rdfs:subClassOf C2004A04997: ;
    skos:definition "Subheading Notes"@en-AU ;
    skos:narrower C2004A04997:103 ;
    skos:prefLabel "Item I195"@en-AU ;
    dcat:accessURL <https://www.legislation.gov.au/C2004A04997/2024-07-01/2024-07-01/text/1/epub/OEBPS/document_2/document_2.html#_Toc171751021> ;
    dcat:landingPage "https://www.legislation.gov.au/C2004A04997/2024-07-01/2024-07-01/text/1/epub/OEBPS/document_2/document_2.html#_Toc171751021"^^xsd:anyURI ;
    dcat:theme legcons:Item .

C2004A04997:196 a legcons:Item,
        C2004A04997:Item,
        owl:Class,
        dcat:Resource ;
    rdfs:label "Item - I196 Additional Note"@en-AU ;
    dct:isPartOf C2004A04997:103 ;
    rdfs:comment "Additional Note - Abrievated Graph Key: I196"@en-AU ;
    rdfs:subClassOf C2004A04997: ;
    skos:definition "Additional Note"@en-AU ;
    skos:narrower C2004A04997:103 ;
    skos:prefLabel "Item I196"@en-AU ;
    dcat:accessURL <https://www.legislation.gov.au/C2004A04997/2024-07-01/2024-07-01/text/1/epub/OEBPS/document_2/document_2.html#_Toc171751022> ;
    dcat:landingPage "https://www.legislation.gov.au/C2004A04997/2024-07-01/2024-07-01/text/1/epub/OEBPS/document_2/document_2.html#_Toc171751022"^^xsd:anyURI ;
    dcat:theme legcons:Item .

C2004A04997:197 a legcons:Volume,
        C2004A04997:Volume,
        owl:Class,
        dcat:Resource ;
    rdfs:label "Volume - V197 Volume 3"@en-AU ;
    dct:hasPart C2004A04997:198 ;
    rdfs:comment "Volume 3 - Abrievated Graph Key: V197"@en-AU ;
    rdfs:subClassOf C2004A04997: ;
    skos:broader C2004A04997:198 ;
    skos:definition "Volume 3"@en-AU ;
    skos:prefLabel "Volume V197"@en-AU ;
    dcat:accessURL <https://www.legislation.gov.au/C2004A04997/2024-07-01/2024-07-01/text/1/epub/OEBPS/document_3/document_3.html> ;
    dcat:landingPage "https://www.legislation.gov.au/C2004A04997/2024-07-01/2024-07-01/text/1/epub/OEBPS/document_3/document_3.html"^^xsd:anyURI ;
    dcat:theme legcons:Volume .

C2004A04997:199 a legcons:Section,
        C2004A04997:Section,
        owl:Class,
        dcat:Resource ;
    rdfs:label "Section - S199 Section VIIPlastics and articles thereof rubber and articles thereof"@en-AU ;
    dct:isPartOf C2004A04997:198 ;
    rdfs:comment "Section VIIPlastics and articles thereof rubber and articles thereof - Abrievated Graph Key: S199"@en-AU ;
    rdfs:subClassOf C2004A04997: ;
    skos:definition "Section VIIPlastics and articles thereof rubber and articles thereof"@en-AU ;
    skos:narrower C2004A04997:198 ;
    skos:prefLabel "Section S199"@en-AU ;
    dcat:accessURL <https://www.legislation.gov.au/C2004A04997/2024-07-01/2024-07-01/text/1/epub/OEBPS/document_3/document_3.html#_Toc171751529> ;
    dcat:landingPage "https://www.legislation.gov.au/C2004A04997/2024-07-01/2024-07-01/text/1/epub/OEBPS/document_3/document_3.html#_Toc171751529"^^xsd:anyURI ;
    dcat:theme legcons:Section .

C2004A04997:20 a legcons:Item,
        C2004A04997:Item,
        owl:Class,
        dcat:Resource ;
    rdfs:label "Item - I20 13 C  When goods are New Zealand originating goods"@en-AU ;
    dct:isPartOf C2004A04997:2 ;
    rdfs:comment "13 C  When goods are New Zealand originating goods - Abrievated Graph Key: I20"@en-AU ;
    rdfs:subClassOf C2004A04997: ;
    skos:definition "13 C  When goods are New Zealand originating goods"@en-AU ;
    skos:narrower C2004A04997:2 ;
    skos:prefLabel "Item I20"@en-AU ;
    dcat:accessURL <https://www.legislation.gov.au/C2004A04997/2024-07-01/2024-07-01/text/1/epub/OEBPS/document_1/document_1.html#_Toc172806520> ;
    dcat:landingPage "https://www.legislation.gov.au/C2004A04997/2024-07-01/2024-07-01/text/1/epub/OEBPS/document_1/document_1.html#_Toc172806520"^^xsd:anyURI ;
    dcat:theme legcons:Item .

C2004A04997:200 a legcons:Item,
        C2004A04997:Item,
        owl:Class,
        dcat:Resource ;
    rdfs:label "Item - I200 Notes"@en-AU ;
    dct:isPartOf C2004A04997:198 ;
    rdfs:comment "Notes - Abrievated Graph Key: I200"@en-AU ;
    rdfs:subClassOf C2004A04997: ;
    skos:definition "Notes"@en-AU ;
    skos:narrower C2004A04997:198 ;
    skos:prefLabel "Item I200"@en-AU ;
    dcat:accessURL <https://www.legislation.gov.au/C2004A04997/2024-07-01/2024-07-01/text/1/epub/OEBPS/document_3/document_3.html#_Toc171751530> ;
    dcat:landingPage "https://www.legislation.gov.au/C2004A04997/2024-07-01/2024-07-01/text/1/epub/OEBPS/document_3/document_3.html#_Toc171751530"^^xsd:anyURI ;
    dcat:theme legcons:Item .

C2004A04997:201 a legcons:Item,
        C2004A04997:Item,
        owl:Class,
        dcat:Resource ;
    rdfs:label "Item - I201 Additional Note"@en-AU ;
    dct:isPartOf C2004A04997:198 ;
    rdfs:comment "Additional Note - Abrievated Graph Key: I201"@en-AU ;
    rdfs:subClassOf C2004A04997: ;
    skos:definition "Additional Note"@en-AU ;
    skos:narrower C2004A04997:198 ;
    skos:prefLabel "Item I201"@en-AU ;
    dcat:accessURL <https://www.legislation.gov.au/C2004A04997/2024-07-01/2024-07-01/text/1/epub/OEBPS/document_3/document_3.html#_Toc171751531> ;
    dcat:landingPage "https://www.legislation.gov.au/C2004A04997/2024-07-01/2024-07-01/text/1/epub/OEBPS/document_3/document_3.html#_Toc171751531"^^xsd:anyURI ;
    dcat:theme legcons:Item .

C2004A04997:202 a legcons:Chapter,
        C2004A04997:Chapter,
        owl:Class,
        dcat:Resource ;
    rdfs:label "Chapter - C202 Chapter 39 Plastics and articles thereof"@en-AU ;
    dct:isPartOf C2004A04997:198 ;
    rdfs:comment "Chapter 39 Plastics and articles thereof - Abrievated Graph Key: C202"@en-AU ;
    rdfs:subClassOf C2004A04997: ;
    skos:definition "Chapter 39 Plastics and articles thereof"@en-AU ;
    skos:narrower C2004A04997:198 ;
    skos:prefLabel "Chapter C202"@en-AU ;
    dcat:accessURL <https://www.legislation.gov.au/C2004A04997/2024-07-01/2024-07-01/text/1/epub/OEBPS/document_3/document_3.html#_Toc171751532> ;
    dcat:landingPage "https://www.legislation.gov.au/C2004A04997/2024-07-01/2024-07-01/text/1/epub/OEBPS/document_3/document_3.html#_Toc171751532"^^xsd:anyURI ;
    dcat:theme legcons:Chapter .

C2004A04997:203 a legcons:Item,
        C2004A04997:Item,
        owl:Class,
        dcat:Resource ;
    rdfs:label "Item - I203 Notes"@en-AU ;
    dct:isPartOf C2004A04997:198 ;
    rdfs:comment "Notes - Abrievated Graph Key: I203"@en-AU ;
    rdfs:subClassOf C2004A04997: ;
    skos:definition "Notes"@en-AU ;
    skos:narrower C2004A04997:198 ;
    skos:prefLabel "Item I203"@en-AU ;
    dcat:accessURL <https://www.legislation.gov.au/C2004A04997/2024-07-01/2024-07-01/text/1/epub/OEBPS/document_3/document_3.html#_Toc171751533> ;
    dcat:landingPage "https://www.legislation.gov.au/C2004A04997/2024-07-01/2024-07-01/text/1/epub/OEBPS/document_3/document_3.html#_Toc171751533"^^xsd:anyURI ;
    dcat:theme legcons:Item .

C2004A04997:204 a legcons:Item,
        C2004A04997:Item,
        owl:Class,
        dcat:Resource ;
    rdfs:label "Item - I204 Subheading Notes"@en-AU ;
    dct:isPartOf C2004A04997:198 ;
    rdfs:comment "Subheading Notes - Abrievated Graph Key: I204"@en-AU ;
    rdfs:subClassOf C2004A04997: ;
    skos:definition "Subheading Notes"@en-AU ;
    skos:narrower C2004A04997:198 ;
    skos:prefLabel "Item I204"@en-AU ;
    dcat:accessURL <https://www.legislation.gov.au/C2004A04997/2024-07-01/2024-07-01/text/1/epub/OEBPS/document_3/document_3.html#_Toc171751534> ;
    dcat:landingPage "https://www.legislation.gov.au/C2004A04997/2024-07-01/2024-07-01/text/1/epub/OEBPS/document_3/document_3.html#_Toc171751534"^^xsd:anyURI ;
    dcat:theme legcons:Item .

C2004A04997:205 a legcons:Item,
        C2004A04997:Item,
        owl:Class,
        dcat:Resource ;
    rdfs:label "Item - I205 Additional Notes"@en-AU ;
    dct:isPartOf C2004A04997:198 ;
    rdfs:comment "Additional Notes - Abrievated Graph Key: I205"@en-AU ;
    rdfs:subClassOf C2004A04997: ;
    skos:definition "Additional Notes"@en-AU ;
    skos:narrower C2004A04997:198 ;
    skos:prefLabel "Item I205"@en-AU ;
    dcat:accessURL <https://www.legislation.gov.au/C2004A04997/2024-07-01/2024-07-01/text/1/epub/OEBPS/document_3/document_3.html#_Toc171751535> ;
    dcat:landingPage "https://www.legislation.gov.au/C2004A04997/2024-07-01/2024-07-01/text/1/epub/OEBPS/document_3/document_3.html#_Toc171751535"^^xsd:anyURI ;
    dcat:theme legcons:Item .

C2004A04997:206 a legcons:Item,
        C2004A04997:Item,
        owl:Class,
        dcat:Resource ;
    rdfs:label "Item - I206 Sub Chapter IPrimary forms"@en-AU ;
    dct:isPartOf C2004A04997:198 ;
    rdfs:comment "Sub Chapter IPrimary forms - Abrievated Graph Key: I206"@en-AU ;
    rdfs:subClassOf C2004A04997: ;
    skos:definition "Sub Chapter IPrimary forms"@en-AU ;
    skos:narrower C2004A04997:198 ;
    skos:prefLabel "Item I206"@en-AU ;
    dcat:accessURL <https://www.legislation.gov.au/C2004A04997/2024-07-01/2024-07-01/text/1/epub/OEBPS/document_3/document_3.html#_Toc171751536> ;
    dcat:landingPage "https://www.legislation.gov.au/C2004A04997/2024-07-01/2024-07-01/text/1/epub/OEBPS/document_3/document_3.html#_Toc171751536"^^xsd:anyURI ;
    dcat:theme legcons:Item .

C2004A04997:207 a legcons:Item,
        C2004A04997:Item,
        owl:Class,
        dcat:Resource ;
    rdfs:label "Item - I207 Sub Chapter IIWaste parings and scrap semi manufactures articles"@en-AU ;
    dct:isPartOf C2004A04997:198 ;
    rdfs:comment "Sub Chapter IIWaste parings and scrap semi manufactures articles - Abrievated Graph Key: I207"@en-AU ;
    rdfs:subClassOf C2004A04997: ;
    skos:definition "Sub Chapter IIWaste parings and scrap semi manufactures articles"@en-AU ;
    skos:narrower C2004A04997:198 ;
    skos:prefLabel "Item I207"@en-AU ;
    dcat:accessURL <https://www.legislation.gov.au/C2004A04997/2024-07-01/2024-07-01/text/1/epub/OEBPS/document_3/document_3.html#_Toc171751537> ;
    dcat:landingPage "https://www.legislation.gov.au/C2004A04997/2024-07-01/2024-07-01/text/1/epub/OEBPS/document_3/document_3.html#_Toc171751537"^^xsd:anyURI ;
    dcat:theme legcons:Item .

C2004A04997:208 a legcons:Chapter,
        C2004A04997:Chapter,
        owl:Class,
        dcat:Resource ;
    rdfs:label "Chapter - C208 Chapter 40 Rubber and articles thereof"@en-AU ;
    dct:isPartOf C2004A04997:198 ;
    rdfs:comment "Chapter 40 Rubber and articles thereof - Abrievated Graph Key: C208"@en-AU ;
    rdfs:subClassOf C2004A04997: ;
    skos:definition "Chapter 40 Rubber and articles thereof"@en-AU ;
    skos:narrower C2004A04997:198 ;
    skos:prefLabel "Chapter C208"@en-AU ;
    dcat:accessURL <https://www.legislation.gov.au/C2004A04997/2024-07-01/2024-07-01/text/1/epub/OEBPS/document_3/document_3.html#_Toc171751538> ;
    dcat:landingPage "https://www.legislation.gov.au/C2004A04997/2024-07-01/2024-07-01/text/1/epub/OEBPS/document_3/document_3.html#_Toc171751538"^^xsd:anyURI ;
    dcat:theme legcons:Chapter .

C2004A04997:209 a legcons:Item,
        C2004A04997:Item,
        owl:Class,
        dcat:Resource ;
    rdfs:label "Item - I209 Notes"@en-AU ;
    dct:isPartOf C2004A04997:198 ;
    rdfs:comment "Notes - Abrievated Graph Key: I209"@en-AU ;
    rdfs:subClassOf C2004A04997: ;
    skos:definition "Notes"@en-AU ;
    skos:narrower C2004A04997:198 ;
    skos:prefLabel "Item I209"@en-AU ;
    dcat:accessURL <https://www.legislation.gov.au/C2004A04997/2024-07-01/2024-07-01/text/1/epub/OEBPS/document_3/document_3.html#_Toc171751539> ;
    dcat:landingPage "https://www.legislation.gov.au/C2004A04997/2024-07-01/2024-07-01/text/1/epub/OEBPS/document_3/document_3.html#_Toc171751539"^^xsd:anyURI ;
    dcat:theme legcons:Item .

C2004A04997:21 a legcons:Item,
        C2004A04997:Item,
        owl:Class,
        dcat:Resource ;
    rdfs:label "Item - I21 13 CA  When goods are Peruvian originating goods"@en-AU ;
    dct:isPartOf C2004A04997:2 ;
    rdfs:comment "13 CA  When goods are Peruvian originating goods - Abrievated Graph Key: I21"@en-AU ;
    rdfs:subClassOf C2004A04997: ;
    skos:definition "13 CA  When goods are Peruvian originating goods"@en-AU ;
    skos:narrower C2004A04997:2 ;
    skos:prefLabel "Item I21"@en-AU ;
    dcat:accessURL <https://www.legislation.gov.au/C2004A04997/2024-07-01/2024-07-01/text/1/epub/OEBPS/document_1/document_1.html#_Toc172806521> ;
    dcat:landingPage "https://www.legislation.gov.au/C2004A04997/2024-07-01/2024-07-01/text/1/epub/OEBPS/document_1/document_1.html#_Toc172806521"^^xsd:anyURI ;
    dcat:theme legcons:Item .

C2004A04997:210 a legcons:Section,
        C2004A04997:Section,
        owl:Class,
        dcat:Resource ;
    rdfs:label "Section - S210 Section VIIIRaw hides and skins leather furskins and articles thereof saddlery and harness travel goods handbags and similar containers articles of animal gut other than silk worm gut"@en-AU ;
    dct:isPartOf C2004A04997:198 ;
    rdfs:comment "Section VIIIRaw hides and skins leather furskins and articles thereof saddlery and harness travel goods handbags and similar containers articles of animal gut other than silk worm gut - Abrievated Graph Key: S210"@en-AU ;
    rdfs:subClassOf C2004A04997: ;
    skos:definition "Section VIIIRaw hides and skins leather furskins and articles thereof saddlery and harness travel goods handbags and similar containers articles of animal gut other than silk worm gut"@en-AU ;
    skos:narrower C2004A04997:198 ;
    skos:prefLabel "Section S210"@en-AU ;
    dcat:accessURL <https://www.legislation.gov.au/C2004A04997/2024-07-01/2024-07-01/text/1/epub/OEBPS/document_3/document_3.html#_Toc171751540> ;
    dcat:landingPage "https://www.legislation.gov.au/C2004A04997/2024-07-01/2024-07-01/text/1/epub/OEBPS/document_3/document_3.html#_Toc171751540"^^xsd:anyURI ;
    dcat:theme legcons:Section .

C2004A04997:211 a legcons:Chapter,
        C2004A04997:Chapter,
        owl:Class,
        dcat:Resource ;
    rdfs:label "Chapter - C211 Chapter 41 Raw hides and skins other than furskins and leather"@en-AU ;
    dct:isPartOf C2004A04997:198 ;
    rdfs:comment "Chapter 41 Raw hides and skins other than furskins and leather - Abrievated Graph Key: C211"@en-AU ;
    rdfs:subClassOf C2004A04997: ;
    skos:definition "Chapter 41 Raw hides and skins other than furskins and leather"@en-AU ;
    skos:narrower C2004A04997:198 ;
    skos:prefLabel "Chapter C211"@en-AU ;
    dcat:accessURL <https://www.legislation.gov.au/C2004A04997/2024-07-01/2024-07-01/text/1/epub/OEBPS/document_3/document_3.html#_Toc171751541> ;
    dcat:landingPage "https://www.legislation.gov.au/C2004A04997/2024-07-01/2024-07-01/text/1/epub/OEBPS/document_3/document_3.html#_Toc171751541"^^xsd:anyURI ;
    dcat:theme legcons:Chapter .

C2004A04997:212 a legcons:Item,
        C2004A04997:Item,
        owl:Class,
        dcat:Resource ;
    rdfs:label "Item - I212 Notes"@en-AU ;
    dct:isPartOf C2004A04997:198 ;
    rdfs:comment "Notes - Abrievated Graph Key: I212"@en-AU ;
    rdfs:subClassOf C2004A04997: ;
    skos:definition "Notes"@en-AU ;
    skos:narrower C2004A04997:198 ;
    skos:prefLabel "Item I212"@en-AU ;
    dcat:accessURL <https://www.legislation.gov.au/C2004A04997/2024-07-01/2024-07-01/text/1/epub/OEBPS/document_3/document_3.html#_Toc171751542> ;
    dcat:landingPage "https://www.legislation.gov.au/C2004A04997/2024-07-01/2024-07-01/text/1/epub/OEBPS/document_3/document_3.html#_Toc171751542"^^xsd:anyURI ;
    dcat:theme legcons:Item .

C2004A04997:213 a legcons:Chapter,
        C2004A04997:Chapter,
        owl:Class,
        dcat:Resource ;
    rdfs:label "Chapter - C213 Chapter 42 Articles of leather saddlery and harness travel goods handbags and similar containers articles of animal gut other than silk worm gut"@en-AU ;
    dct:isPartOf C2004A04997:198 ;
    rdfs:comment "Chapter 42 Articles of leather saddlery and harness travel goods handbags and similar containers articles of animal gut other than silk worm gut - Abrievated Graph Key: C213"@en-AU ;
    rdfs:subClassOf C2004A04997: ;
    skos:definition "Chapter 42 Articles of leather saddlery and harness travel goods handbags and similar containers articles of animal gut other than silk worm gut"@en-AU ;
    skos:narrower C2004A04997:198 ;
    skos:prefLabel "Chapter C213"@en-AU ;
    dcat:accessURL <https://www.legislation.gov.au/C2004A04997/2024-07-01/2024-07-01/text/1/epub/OEBPS/document_3/document_3.html#_Toc171751543> ;
    dcat:landingPage "https://www.legislation.gov.au/C2004A04997/2024-07-01/2024-07-01/text/1/epub/OEBPS/document_3/document_3.html#_Toc171751543"^^xsd:anyURI ;
    dcat:theme legcons:Chapter .

C2004A04997:214 a legcons:Item,
        C2004A04997:Item,
        owl:Class,
        dcat:Resource ;
    rdfs:label "Item - I214 Notes"@en-AU ;
    dct:isPartOf C2004A04997:198 ;
    rdfs:comment "Notes - Abrievated Graph Key: I214"@en-AU ;
    rdfs:subClassOf C2004A04997: ;
    skos:definition "Notes"@en-AU ;
    skos:narrower C2004A04997:198 ;
    skos:prefLabel "Item I214"@en-AU ;
    dcat:accessURL <https://www.legislation.gov.au/C2004A04997/2024-07-01/2024-07-01/text/1/epub/OEBPS/document_3/document_3.html#_Toc171751544> ;
    dcat:landingPage "https://www.legislation.gov.au/C2004A04997/2024-07-01/2024-07-01/text/1/epub/OEBPS/document_3/document_3.html#_Toc171751544"^^xsd:anyURI ;
    dcat:theme legcons:Item .

C2004A04997:215 a legcons:Chapter,
        C2004A04997:Chapter,
        owl:Class,
        dcat:Resource ;
    rdfs:label "Chapter - C215 Chapter 43 Furskins and artificial fur manufactures thereof"@en-AU ;
    dct:isPartOf C2004A04997:198 ;
    rdfs:comment "Chapter 43 Furskins and artificial fur manufactures thereof - Abrievated Graph Key: C215"@en-AU ;
    rdfs:subClassOf C2004A04997: ;
    skos:definition "Chapter 43 Furskins and artificial fur manufactures thereof"@en-AU ;
    skos:narrower C2004A04997:198 ;
    skos:prefLabel "Chapter C215"@en-AU ;
    dcat:accessURL <https://www.legislation.gov.au/C2004A04997/2024-07-01/2024-07-01/text/1/epub/OEBPS/document_3/document_3.html#_Toc171751545> ;
    dcat:landingPage "https://www.legislation.gov.au/C2004A04997/2024-07-01/2024-07-01/text/1/epub/OEBPS/document_3/document_3.html#_Toc171751545"^^xsd:anyURI ;
    dcat:theme legcons:Chapter .

C2004A04997:216 a legcons:Item,
        C2004A04997:Item,
        owl:Class,
        dcat:Resource ;
    rdfs:label "Item - I216 Notes"@en-AU ;
    dct:isPartOf C2004A04997:198 ;
    rdfs:comment "Notes - Abrievated Graph Key: I216"@en-AU ;
    rdfs:subClassOf C2004A04997: ;
    skos:definition "Notes"@en-AU ;
    skos:narrower C2004A04997:198 ;
    skos:prefLabel "Item I216"@en-AU ;
    dcat:accessURL <https://www.legislation.gov.au/C2004A04997/2024-07-01/2024-07-01/text/1/epub/OEBPS/document_3/document_3.html#_Toc171751546> ;
    dcat:landingPage "https://www.legislation.gov.au/C2004A04997/2024-07-01/2024-07-01/text/1/epub/OEBPS/document_3/document_3.html#_Toc171751546"^^xsd:anyURI ;
    dcat:theme legcons:Item .

C2004A04997:217 a legcons:Section,
        C2004A04997:Section,
        owl:Class,
        dcat:Resource ;
    rdfs:label "Section - S217 Section IXWood and articles of wood wood charcoal cork and articles of cork manufactures of straw of esparto or of other plaiting materials basketware and wickerwork"@en-AU ;
    dct:isPartOf C2004A04997:198 ;
    rdfs:comment "Section IXWood and articles of wood wood charcoal cork and articles of cork manufactures of straw of esparto or of other plaiting materials basketware and wickerwork - Abrievated Graph Key: S217"@en-AU ;
    rdfs:subClassOf C2004A04997: ;
    skos:definition "Section IXWood and articles of wood wood charcoal cork and articles of cork manufactures of straw of esparto or of other plaiting materials basketware and wickerwork"@en-AU ;
    skos:narrower C2004A04997:198 ;
    skos:prefLabel "Section S217"@en-AU ;
    dcat:accessURL <https://www.legislation.gov.au/C2004A04997/2024-07-01/2024-07-01/text/1/epub/OEBPS/document_3/document_3.html#_Toc171751547> ;
    dcat:landingPage "https://www.legislation.gov.au/C2004A04997/2024-07-01/2024-07-01/text/1/epub/OEBPS/document_3/document_3.html#_Toc171751547"^^xsd:anyURI ;
    dcat:theme legcons:Section .

C2004A04997:218 a legcons:Chapter,
        C2004A04997:Chapter,
        owl:Class,
        dcat:Resource ;
    rdfs:label "Chapter - C218 Chapter 44 Wood and articles of wood wood charcoal"@en-AU ;
    dct:isPartOf C2004A04997:198 ;
    rdfs:comment "Chapter 44 Wood and articles of wood wood charcoal - Abrievated Graph Key: C218"@en-AU ;
    rdfs:subClassOf C2004A04997: ;
    skos:definition "Chapter 44 Wood and articles of wood wood charcoal"@en-AU ;
    skos:narrower C2004A04997:198 ;
    skos:prefLabel "Chapter C218"@en-AU ;
    dcat:accessURL <https://www.legislation.gov.au/C2004A04997/2024-07-01/2024-07-01/text/1/epub/OEBPS/document_3/document_3.html#_Toc171751548> ;
    dcat:landingPage "https://www.legislation.gov.au/C2004A04997/2024-07-01/2024-07-01/text/1/epub/OEBPS/document_3/document_3.html#_Toc171751548"^^xsd:anyURI ;
    dcat:theme legcons:Chapter .

C2004A04997:219 a legcons:Item,
        C2004A04997:Item,
        owl:Class,
        dcat:Resource ;
    rdfs:label "Item - I219 Notes"@en-AU ;
    dct:isPartOf C2004A04997:198 ;
    rdfs:comment "Notes - Abrievated Graph Key: I219"@en-AU ;
    rdfs:subClassOf C2004A04997: ;
    skos:definition "Notes"@en-AU ;
    skos:narrower C2004A04997:198 ;
    skos:prefLabel "Item I219"@en-AU ;
    dcat:accessURL <https://www.legislation.gov.au/C2004A04997/2024-07-01/2024-07-01/text/1/epub/OEBPS/document_3/document_3.html#_Toc171751549> ;
    dcat:landingPage "https://www.legislation.gov.au/C2004A04997/2024-07-01/2024-07-01/text/1/epub/OEBPS/document_3/document_3.html#_Toc171751549"^^xsd:anyURI ;
    dcat:theme legcons:Item .

C2004A04997:22 a legcons:Item,
        C2004A04997:Item,
        owl:Class,
        dcat:Resource ;
    rdfs:label "Item - I22 13 D  When goods are Chilean originating goods"@en-AU ;
    dct:isPartOf C2004A04997:2 ;
    rdfs:comment "13 D  When goods are Chilean originating goods - Abrievated Graph Key: I22"@en-AU ;
    rdfs:subClassOf C2004A04997: ;
    skos:definition "13 D  When goods are Chilean originating goods"@en-AU ;
    skos:narrower C2004A04997:2 ;
    skos:prefLabel "Item I22"@en-AU ;
    dcat:accessURL <https://www.legislation.gov.au/C2004A04997/2024-07-01/2024-07-01/text/1/epub/OEBPS/document_1/document_1.html#_Toc172806522> ;
    dcat:landingPage "https://www.legislation.gov.au/C2004A04997/2024-07-01/2024-07-01/text/1/epub/OEBPS/document_1/document_1.html#_Toc172806522"^^xsd:anyURI ;
    dcat:theme legcons:Item .

C2004A04997:220 a legcons:Item,
        C2004A04997:Item,
        owl:Class,
        dcat:Resource ;
    rdfs:label "Item - I220 Subheading Notes"@en-AU ;
    dct:isPartOf C2004A04997:198 ;
    rdfs:comment "Subheading Notes - Abrievated Graph Key: I220"@en-AU ;
    rdfs:subClassOf C2004A04997: ;
    skos:definition "Subheading Notes"@en-AU ;
    skos:narrower C2004A04997:198 ;
    skos:prefLabel "Item I220"@en-AU ;
    dcat:accessURL <https://www.legislation.gov.au/C2004A04997/2024-07-01/2024-07-01/text/1/epub/OEBPS/document_3/document_3.html#_Toc171751550> ;
    dcat:landingPage "https://www.legislation.gov.au/C2004A04997/2024-07-01/2024-07-01/text/1/epub/OEBPS/document_3/document_3.html#_Toc171751550"^^xsd:anyURI ;
    dcat:theme legcons:Item .

C2004A04997:221 a legcons:Item,
        C2004A04997:Item,
        owl:Class,
        dcat:Resource ;
    rdfs:label "Item - I221 Additional Notes"@en-AU ;
    dct:isPartOf C2004A04997:198 ;
    rdfs:comment "Additional Notes - Abrievated Graph Key: I221"@en-AU ;
    rdfs:subClassOf C2004A04997: ;
    skos:definition "Additional Notes"@en-AU ;
    skos:narrower C2004A04997:198 ;
    skos:prefLabel "Item I221"@en-AU ;
    dcat:accessURL <https://www.legislation.gov.au/C2004A04997/2024-07-01/2024-07-01/text/1/epub/OEBPS/document_3/document_3.html#_Toc171751551> ;
    dcat:landingPage "https://www.legislation.gov.au/C2004A04997/2024-07-01/2024-07-01/text/1/epub/OEBPS/document_3/document_3.html#_Toc171751551"^^xsd:anyURI ;
    dcat:theme legcons:Item .

C2004A04997:222 a legcons:Chapter,
        C2004A04997:Chapter,
        owl:Class,
        dcat:Resource ;
    rdfs:label "Chapter - C222 Chapter 45 Cork and articles of cork"@en-AU ;
    dct:isPartOf C2004A04997:198 ;
    rdfs:comment "Chapter 45 Cork and articles of cork - Abrievated Graph Key: C222"@en-AU ;
    rdfs:subClassOf C2004A04997: ;
    skos:definition "Chapter 45 Cork and articles of cork"@en-AU ;
    skos:narrower C2004A04997:198 ;
    skos:prefLabel "Chapter C222"@en-AU ;
    dcat:accessURL <https://www.legislation.gov.au/C2004A04997/2024-07-01/2024-07-01/text/1/epub/OEBPS/document_3/document_3.html#_Toc171751552> ;
    dcat:landingPage "https://www.legislation.gov.au/C2004A04997/2024-07-01/2024-07-01/text/1/epub/OEBPS/document_3/document_3.html#_Toc171751552"^^xsd:anyURI ;
    dcat:theme legcons:Chapter .

C2004A04997:223 a legcons:Item,
        C2004A04997:Item,
        owl:Class,
        dcat:Resource ;
    rdfs:label "Item - I223 Note"@en-AU ;
    dct:isPartOf C2004A04997:198 ;
    rdfs:comment "Note - Abrievated Graph Key: I223"@en-AU ;
    rdfs:subClassOf C2004A04997: ;
    skos:definition "Note"@en-AU ;
    skos:narrower C2004A04997:198 ;
    skos:prefLabel "Item I223"@en-AU ;
    dcat:accessURL <https://www.legislation.gov.au/C2004A04997/2024-07-01/2024-07-01/text/1/epub/OEBPS/document_3/document_3.html#_Toc171751553> ;
    dcat:landingPage "https://www.legislation.gov.au/C2004A04997/2024-07-01/2024-07-01/text/1/epub/OEBPS/document_3/document_3.html#_Toc171751553"^^xsd:anyURI ;
    dcat:theme legcons:Item .

C2004A04997:224 a legcons:Chapter,
        C2004A04997:Chapter,
        owl:Class,
        dcat:Resource ;
    rdfs:label "Chapter - C224 Chapter 46 Manufactures of straw of esparto or of other plaiting materials basketware and wickerwork"@en-AU ;
    dct:isPartOf C2004A04997:198 ;
    rdfs:comment "Chapter 46 Manufactures of straw of esparto or of other plaiting materials basketware and wickerwork - Abrievated Graph Key: C224"@en-AU ;
    rdfs:subClassOf C2004A04997: ;
    skos:definition "Chapter 46 Manufactures of straw of esparto or of other plaiting materials basketware and wickerwork"@en-AU ;
    skos:narrower C2004A04997:198 ;
    skos:prefLabel "Chapter C224"@en-AU ;
    dcat:accessURL <https://www.legislation.gov.au/C2004A04997/2024-07-01/2024-07-01/text/1/epub/OEBPS/document_3/document_3.html#_Toc171751554> ;
    dcat:landingPage "https://www.legislation.gov.au/C2004A04997/2024-07-01/2024-07-01/text/1/epub/OEBPS/document_3/document_3.html#_Toc171751554"^^xsd:anyURI ;
    dcat:theme legcons:Chapter .

C2004A04997:225 a legcons:Item,
        C2004A04997:Item,
        owl:Class,
        dcat:Resource ;
    rdfs:label "Item - I225 Notes"@en-AU ;
    dct:isPartOf C2004A04997:198 ;
    rdfs:comment "Notes - Abrievated Graph Key: I225"@en-AU ;
    rdfs:subClassOf C2004A04997: ;
    skos:definition "Notes"@en-AU ;
    skos:narrower C2004A04997:198 ;
    skos:prefLabel "Item I225"@en-AU ;
    dcat:accessURL <https://www.legislation.gov.au/C2004A04997/2024-07-01/2024-07-01/text/1/epub/OEBPS/document_3/document_3.html#_Toc171751555> ;
    dcat:landingPage "https://www.legislation.gov.au/C2004A04997/2024-07-01/2024-07-01/text/1/epub/OEBPS/document_3/document_3.html#_Toc171751555"^^xsd:anyURI ;
    dcat:theme legcons:Item .

C2004A04997:226 a legcons:Section,
        C2004A04997:Section,
        owl:Class,
        dcat:Resource ;
    rdfs:label "Section - S226 Section XPulp of wood or of other fibrous cellulosic material recovered waste and scrap paper or paperboard paper and paperboard and articles thereof"@en-AU ;
    dct:isPartOf C2004A04997:198 ;
    rdfs:comment "Section XPulp of wood or of other fibrous cellulosic material recovered waste and scrap paper or paperboard paper and paperboard and articles thereof - Abrievated Graph Key: S226"@en-AU ;
    rdfs:subClassOf C2004A04997: ;
    skos:definition "Section XPulp of wood or of other fibrous cellulosic material recovered waste and scrap paper or paperboard paper and paperboard and articles thereof"@en-AU ;
    skos:narrower C2004A04997:198 ;
    skos:prefLabel "Section S226"@en-AU ;
    dcat:accessURL <https://www.legislation.gov.au/C2004A04997/2024-07-01/2024-07-01/text/1/epub/OEBPS/document_3/document_3.html#_Toc171751556> ;
    dcat:landingPage "https://www.legislation.gov.au/C2004A04997/2024-07-01/2024-07-01/text/1/epub/OEBPS/document_3/document_3.html#_Toc171751556"^^xsd:anyURI ;
    dcat:theme legcons:Section .

C2004A04997:227 a legcons:Chapter,
        C2004A04997:Chapter,
        owl:Class,
        dcat:Resource ;
    rdfs:label "Chapter - C227 Chapter 47 Pulp of wood or of other fibrous cellulosic material recovered waste and scrap paper or paperboard"@en-AU ;
    dct:isPartOf C2004A04997:198 ;
    rdfs:comment "Chapter 47 Pulp of wood or of other fibrous cellulosic material recovered waste and scrap paper or paperboard - Abrievated Graph Key: C227"@en-AU ;
    rdfs:subClassOf C2004A04997: ;
    skos:definition "Chapter 47 Pulp of wood or of other fibrous cellulosic material recovered waste and scrap paper or paperboard"@en-AU ;
    skos:narrower C2004A04997:198 ;
    skos:prefLabel "Chapter C227"@en-AU ;
    dcat:accessURL <https://www.legislation.gov.au/C2004A04997/2024-07-01/2024-07-01/text/1/epub/OEBPS/document_3/document_3.html#_Toc171751557> ;
    dcat:landingPage "https://www.legislation.gov.au/C2004A04997/2024-07-01/2024-07-01/text/1/epub/OEBPS/document_3/document_3.html#_Toc171751557"^^xsd:anyURI ;
    dcat:theme legcons:Chapter .

C2004A04997:228 a legcons:Item,
        C2004A04997:Item,
        owl:Class,
        dcat:Resource ;
    rdfs:label "Item - I228 Note"@en-AU ;
    dct:isPartOf C2004A04997:198 ;
    rdfs:comment "Note - Abrievated Graph Key: I228"@en-AU ;
    rdfs:subClassOf C2004A04997: ;
    skos:definition "Note"@en-AU ;
    skos:narrower C2004A04997:198 ;
    skos:prefLabel "Item I228"@en-AU ;
    dcat:accessURL <https://www.legislation.gov.au/C2004A04997/2024-07-01/2024-07-01/text/1/epub/OEBPS/document_3/document_3.html#_Toc171751558> ;
    dcat:landingPage "https://www.legislation.gov.au/C2004A04997/2024-07-01/2024-07-01/text/1/epub/OEBPS/document_3/document_3.html#_Toc171751558"^^xsd:anyURI ;
    dcat:theme legcons:Item .

C2004A04997:229 a legcons:Chapter,
        C2004A04997:Chapter,
        owl:Class,
        dcat:Resource ;
    rdfs:label "Chapter - C229 Chapter 48 Paper and paperboard articles of paper pulp of paper or of paperboard"@en-AU ;
    dct:isPartOf C2004A04997:198 ;
    rdfs:comment "Chapter 48 Paper and paperboard articles of paper pulp of paper or of paperboard - Abrievated Graph Key: C229"@en-AU ;
    rdfs:subClassOf C2004A04997: ;
    skos:definition "Chapter 48 Paper and paperboard articles of paper pulp of paper or of paperboard"@en-AU ;
    skos:narrower C2004A04997:198 ;
    skos:prefLabel "Chapter C229"@en-AU ;
    dcat:accessURL <https://www.legislation.gov.au/C2004A04997/2024-07-01/2024-07-01/text/1/epub/OEBPS/document_3/document_3.html#_Toc171751559> ;
    dcat:landingPage "https://www.legislation.gov.au/C2004A04997/2024-07-01/2024-07-01/text/1/epub/OEBPS/document_3/document_3.html#_Toc171751559"^^xsd:anyURI ;
    dcat:theme legcons:Chapter .

C2004A04997:23 a legcons:Item,
        C2004A04997:Item,
        owl:Class,
        dcat:Resource ;
    rdfs:label "Item - I23 13 E  When goods are ASEAN Australia New Zealand AANZ originating goods"@en-AU ;
    dct:isPartOf C2004A04997:2 ;
    rdfs:comment "13 E  When goods are ASEAN Australia New Zealand AANZ originating goods - Abrievated Graph Key: I23"@en-AU ;
    rdfs:subClassOf C2004A04997: ;
    skos:definition "13 E  When goods are ASEAN Australia New Zealand AANZ originating goods"@en-AU ;
    skos:narrower C2004A04997:2 ;
    skos:prefLabel "Item I23"@en-AU ;
    dcat:accessURL <https://www.legislation.gov.au/C2004A04997/2024-07-01/2024-07-01/text/1/epub/OEBPS/document_1/document_1.html#_Toc172806523> ;
    dcat:landingPage "https://www.legislation.gov.au/C2004A04997/2024-07-01/2024-07-01/text/1/epub/OEBPS/document_1/document_1.html#_Toc172806523"^^xsd:anyURI ;
    dcat:theme legcons:Item .

C2004A04997:230 a legcons:Item,
        C2004A04997:Item,
        owl:Class,
        dcat:Resource ;
    rdfs:label "Item - I230 Notes"@en-AU ;
    dct:isPartOf C2004A04997:198 ;
    rdfs:comment "Notes - Abrievated Graph Key: I230"@en-AU ;
    rdfs:subClassOf C2004A04997: ;
    skos:definition "Notes"@en-AU ;
    skos:narrower C2004A04997:198 ;
    skos:prefLabel "Item I230"@en-AU ;
    dcat:accessURL <https://www.legislation.gov.au/C2004A04997/2024-07-01/2024-07-01/text/1/epub/OEBPS/document_3/document_3.html#_Toc171751560> ;
    dcat:landingPage "https://www.legislation.gov.au/C2004A04997/2024-07-01/2024-07-01/text/1/epub/OEBPS/document_3/document_3.html#_Toc171751560"^^xsd:anyURI ;
    dcat:theme legcons:Item .

C2004A04997:231 a legcons:Item,
        C2004A04997:Item,
        owl:Class,
        dcat:Resource ;
    rdfs:label "Item - I231 Subheading Notes"@en-AU ;
    dct:isPartOf C2004A04997:198 ;
    rdfs:comment "Subheading Notes - Abrievated Graph Key: I231"@en-AU ;
    rdfs:subClassOf C2004A04997: ;
    skos:definition "Subheading Notes"@en-AU ;
    skos:narrower C2004A04997:198 ;
    skos:prefLabel "Item I231"@en-AU ;
    dcat:accessURL <https://www.legislation.gov.au/C2004A04997/2024-07-01/2024-07-01/text/1/epub/OEBPS/document_3/document_3.html#_Toc171751561> ;
    dcat:landingPage "https://www.legislation.gov.au/C2004A04997/2024-07-01/2024-07-01/text/1/epub/OEBPS/document_3/document_3.html#_Toc171751561"^^xsd:anyURI ;
    dcat:theme legcons:Item .

C2004A04997:232 a legcons:Item,
        C2004A04997:Item,
        owl:Class,
        dcat:Resource ;
    rdfs:label "Item - I232 Additional Notes"@en-AU ;
    dct:isPartOf C2004A04997:198 ;
    rdfs:comment "Additional Notes - Abrievated Graph Key: I232"@en-AU ;
    rdfs:subClassOf C2004A04997: ;
    skos:definition "Additional Notes"@en-AU ;
    skos:narrower C2004A04997:198 ;
    skos:prefLabel "Item I232"@en-AU ;
    dcat:accessURL <https://www.legislation.gov.au/C2004A04997/2024-07-01/2024-07-01/text/1/epub/OEBPS/document_3/document_3.html#_Toc171751562> ;
    dcat:landingPage "https://www.legislation.gov.au/C2004A04997/2024-07-01/2024-07-01/text/1/epub/OEBPS/document_3/document_3.html#_Toc171751562"^^xsd:anyURI ;
    dcat:theme legcons:Item .

C2004A04997:233 a legcons:Chapter,
        C2004A04997:Chapter,
        owl:Class,
        dcat:Resource ;
    rdfs:label "Chapter - C233 Chapter 49 Printed books newspapers pictures and other products of the printing industry manuscripts typescripts and plans"@en-AU ;
    dct:isPartOf C2004A04997:198 ;
    rdfs:comment "Chapter 49 Printed books newspapers pictures and other products of the printing industry manuscripts typescripts and plans - Abrievated Graph Key: C233"@en-AU ;
    rdfs:subClassOf C2004A04997: ;
    skos:definition "Chapter 49 Printed books newspapers pictures and other products of the printing industry manuscripts typescripts and plans"@en-AU ;
    skos:narrower C2004A04997:198 ;
    skos:prefLabel "Chapter C233"@en-AU ;
    dcat:accessURL <https://www.legislation.gov.au/C2004A04997/2024-07-01/2024-07-01/text/1/epub/OEBPS/document_3/document_3.html#_Toc171751563> ;
    dcat:landingPage "https://www.legislation.gov.au/C2004A04997/2024-07-01/2024-07-01/text/1/epub/OEBPS/document_3/document_3.html#_Toc171751563"^^xsd:anyURI ;
    dcat:theme legcons:Chapter .

C2004A04997:234 a legcons:Item,
        C2004A04997:Item,
        owl:Class,
        dcat:Resource ;
    rdfs:label "Item - I234 Notes"@en-AU ;
    dct:isPartOf C2004A04997:198 ;
    rdfs:comment "Notes - Abrievated Graph Key: I234"@en-AU ;
    rdfs:subClassOf C2004A04997: ;
    skos:definition "Notes"@en-AU ;
    skos:narrower C2004A04997:198 ;
    skos:prefLabel "Item I234"@en-AU ;
    dcat:accessURL <https://www.legislation.gov.au/C2004A04997/2024-07-01/2024-07-01/text/1/epub/OEBPS/document_3/document_3.html#_Toc171751564> ;
    dcat:landingPage "https://www.legislation.gov.au/C2004A04997/2024-07-01/2024-07-01/text/1/epub/OEBPS/document_3/document_3.html#_Toc171751564"^^xsd:anyURI ;
    dcat:theme legcons:Item .

C2004A04997:235 a legcons:Section,
        C2004A04997:Section,
        owl:Class,
        dcat:Resource ;
    rdfs:label "Section - S235 Section XITextiles and textile articles"@en-AU ;
    dct:isPartOf C2004A04997:198 ;
    rdfs:comment "Section XITextiles and textile articles - Abrievated Graph Key: S235"@en-AU ;
    rdfs:subClassOf C2004A04997: ;
    skos:definition "Section XITextiles and textile articles"@en-AU ;
    skos:narrower C2004A04997:198 ;
    skos:prefLabel "Section S235"@en-AU ;
    dcat:accessURL <https://www.legislation.gov.au/C2004A04997/2024-07-01/2024-07-01/text/1/epub/OEBPS/document_3/document_3.html#_Toc171751565> ;
    dcat:landingPage "https://www.legislation.gov.au/C2004A04997/2024-07-01/2024-07-01/text/1/epub/OEBPS/document_3/document_3.html#_Toc171751565"^^xsd:anyURI ;
    dcat:theme legcons:Section .

C2004A04997:236 a legcons:Item,
        C2004A04997:Item,
        owl:Class,
        dcat:Resource ;
    rdfs:label "Item - I236 Notes"@en-AU ;
    dct:isPartOf C2004A04997:198 ;
    rdfs:comment "Notes - Abrievated Graph Key: I236"@en-AU ;
    rdfs:subClassOf C2004A04997: ;
    skos:definition "Notes"@en-AU ;
    skos:narrower C2004A04997:198 ;
    skos:prefLabel "Item I236"@en-AU ;
    dcat:accessURL <https://www.legislation.gov.au/C2004A04997/2024-07-01/2024-07-01/text/1/epub/OEBPS/document_3/document_3.html#_Toc171751566> ;
    dcat:landingPage "https://www.legislation.gov.au/C2004A04997/2024-07-01/2024-07-01/text/1/epub/OEBPS/document_3/document_3.html#_Toc171751566"^^xsd:anyURI ;
    dcat:theme legcons:Item .

C2004A04997:237 a legcons:Item,
        C2004A04997:Item,
        owl:Class,
        dcat:Resource ;
    rdfs:label "Item - I237 Subheading Notes"@en-AU ;
    dct:isPartOf C2004A04997:198 ;
    rdfs:comment "Subheading Notes - Abrievated Graph Key: I237"@en-AU ;
    rdfs:subClassOf C2004A04997: ;
    skos:definition "Subheading Notes"@en-AU ;
    skos:narrower C2004A04997:198 ;
    skos:prefLabel "Item I237"@en-AU ;
    dcat:accessURL <https://www.legislation.gov.au/C2004A04997/2024-07-01/2024-07-01/text/1/epub/OEBPS/document_3/document_3.html#_Toc171751567> ;
    dcat:landingPage "https://www.legislation.gov.au/C2004A04997/2024-07-01/2024-07-01/text/1/epub/OEBPS/document_3/document_3.html#_Toc171751567"^^xsd:anyURI ;
    dcat:theme legcons:Item .

C2004A04997:238 a legcons:Item,
        C2004A04997:Item,
        owl:Class,
        dcat:Resource ;
    rdfs:label "Item - I238 Additional Notes"@en-AU ;
    dct:isPartOf C2004A04997:198 ;
    rdfs:comment "Additional Notes - Abrievated Graph Key: I238"@en-AU ;
    rdfs:subClassOf C2004A04997: ;
    skos:definition "Additional Notes"@en-AU ;
    skos:narrower C2004A04997:198 ;
    skos:prefLabel "Item I238"@en-AU ;
    dcat:accessURL <https://www.legislation.gov.au/C2004A04997/2024-07-01/2024-07-01/text/1/epub/OEBPS/document_3/document_3.html#_Toc171751568> ;
    dcat:landingPage "https://www.legislation.gov.au/C2004A04997/2024-07-01/2024-07-01/text/1/epub/OEBPS/document_3/document_3.html#_Toc171751568"^^xsd:anyURI ;
    dcat:theme legcons:Item .

C2004A04997:239 a legcons:Chapter,
        C2004A04997:Chapter,
        owl:Class,
        dcat:Resource ;
    rdfs:label "Chapter - C239 Chapter 50 Silk"@en-AU ;
    dct:isPartOf C2004A04997:198 ;
    rdfs:comment "Chapter 50 Silk - Abrievated Graph Key: C239"@en-AU ;
    rdfs:subClassOf C2004A04997: ;
    skos:definition "Chapter 50 Silk"@en-AU ;
    skos:narrower C2004A04997:198 ;
    skos:prefLabel "Chapter C239"@en-AU ;
    dcat:accessURL <https://www.legislation.gov.au/C2004A04997/2024-07-01/2024-07-01/text/1/epub/OEBPS/document_3/document_3.html#_Toc171751569> ;
    dcat:landingPage "https://www.legislation.gov.au/C2004A04997/2024-07-01/2024-07-01/text/1/epub/OEBPS/document_3/document_3.html#_Toc171751569"^^xsd:anyURI ;
    dcat:theme legcons:Chapter .

C2004A04997:24 a legcons:Item,
        C2004A04997:Item,
        owl:Class,
        dcat:Resource ;
    rdfs:label "Item - I24 13 EA  When goods are Pacific Islands originating goods"@en-AU ;
    dct:isPartOf C2004A04997:2 ;
    rdfs:comment "13 EA  When goods are Pacific Islands originating goods - Abrievated Graph Key: I24"@en-AU ;
    rdfs:subClassOf C2004A04997: ;
    skos:definition "13 EA  When goods are Pacific Islands originating goods"@en-AU ;
    skos:narrower C2004A04997:2 ;
    skos:prefLabel "Item I24"@en-AU ;
    dcat:accessURL <https://www.legislation.gov.au/C2004A04997/2024-07-01/2024-07-01/text/1/epub/OEBPS/document_1/document_1.html#_Toc172806524> ;
    dcat:landingPage "https://www.legislation.gov.au/C2004A04997/2024-07-01/2024-07-01/text/1/epub/OEBPS/document_1/document_1.html#_Toc172806524"^^xsd:anyURI ;
    dcat:theme legcons:Item .

C2004A04997:240 a legcons:Chapter,
        C2004A04997:Chapter,
        owl:Class,
        dcat:Resource ;
    rdfs:label "Chapter - C240 Chapter 51 Wool fine or coarse animal hair horsehair yarn and woven fabric"@en-AU ;
    dct:isPartOf C2004A04997:198 ;
    rdfs:comment "Chapter 51 Wool fine or coarse animal hair horsehair yarn and woven fabric - Abrievated Graph Key: C240"@en-AU ;
    rdfs:subClassOf C2004A04997: ;
    skos:definition "Chapter 51 Wool fine or coarse animal hair horsehair yarn and woven fabric"@en-AU ;
    skos:narrower C2004A04997:198 ;
    skos:prefLabel "Chapter C240"@en-AU ;
    dcat:accessURL <https://www.legislation.gov.au/C2004A04997/2024-07-01/2024-07-01/text/1/epub/OEBPS/document_3/document_3.html#_Toc171751570> ;
    dcat:landingPage "https://www.legislation.gov.au/C2004A04997/2024-07-01/2024-07-01/text/1/epub/OEBPS/document_3/document_3.html#_Toc171751570"^^xsd:anyURI ;
    dcat:theme legcons:Chapter .

C2004A04997:241 a legcons:Item,
        C2004A04997:Item,
        owl:Class,
        dcat:Resource ;
    rdfs:label "Item - I241 Note"@en-AU ;
    dct:isPartOf C2004A04997:198 ;
    rdfs:comment "Note - Abrievated Graph Key: I241"@en-AU ;
    rdfs:subClassOf C2004A04997: ;
    skos:definition "Note"@en-AU ;
    skos:narrower C2004A04997:198 ;
    skos:prefLabel "Item I241"@en-AU ;
    dcat:accessURL <https://www.legislation.gov.au/C2004A04997/2024-07-01/2024-07-01/text/1/epub/OEBPS/document_3/document_3.html#_Toc171751571> ;
    dcat:landingPage "https://www.legislation.gov.au/C2004A04997/2024-07-01/2024-07-01/text/1/epub/OEBPS/document_3/document_3.html#_Toc171751571"^^xsd:anyURI ;
    dcat:theme legcons:Item .

C2004A04997:242 a legcons:Chapter,
        C2004A04997:Chapter,
        owl:Class,
        dcat:Resource ;
    rdfs:label "Chapter - C242 Chapter 52 Cotton"@en-AU ;
    dct:isPartOf C2004A04997:198 ;
    rdfs:comment "Chapter 52 Cotton - Abrievated Graph Key: C242"@en-AU ;
    rdfs:subClassOf C2004A04997: ;
    skos:definition "Chapter 52 Cotton"@en-AU ;
    skos:narrower C2004A04997:198 ;
    skos:prefLabel "Chapter C242"@en-AU ;
    dcat:accessURL <https://www.legislation.gov.au/C2004A04997/2024-07-01/2024-07-01/text/1/epub/OEBPS/document_3/document_3.html#_Toc171751572> ;
    dcat:landingPage "https://www.legislation.gov.au/C2004A04997/2024-07-01/2024-07-01/text/1/epub/OEBPS/document_3/document_3.html#_Toc171751572"^^xsd:anyURI ;
    dcat:theme legcons:Chapter .

C2004A04997:243 a legcons:Item,
        C2004A04997:Item,
        owl:Class,
        dcat:Resource ;
    rdfs:label "Item - I243 Subheading Note"@en-AU ;
    dct:isPartOf C2004A04997:198 ;
    rdfs:comment "Subheading Note - Abrievated Graph Key: I243"@en-AU ;
    rdfs:subClassOf C2004A04997: ;
    skos:definition "Subheading Note"@en-AU ;
    skos:narrower C2004A04997:198 ;
    skos:prefLabel "Item I243"@en-AU ;
    dcat:accessURL <https://www.legislation.gov.au/C2004A04997/2024-07-01/2024-07-01/text/1/epub/OEBPS/document_3/document_3.html#_Toc171751573> ;
    dcat:landingPage "https://www.legislation.gov.au/C2004A04997/2024-07-01/2024-07-01/text/1/epub/OEBPS/document_3/document_3.html#_Toc171751573"^^xsd:anyURI ;
    dcat:theme legcons:Item .

C2004A04997:244 a legcons:Chapter,
        C2004A04997:Chapter,
        owl:Class,
        dcat:Resource ;
    rdfs:label "Chapter - C244 Chapter 53 Other vegetable textile fibres paper yarn and woven fabrics of paper yarn"@en-AU ;
    dct:isPartOf C2004A04997:198 ;
    rdfs:comment "Chapter 53 Other vegetable textile fibres paper yarn and woven fabrics of paper yarn - Abrievated Graph Key: C244"@en-AU ;
    rdfs:subClassOf C2004A04997: ;
    skos:definition "Chapter 53 Other vegetable textile fibres paper yarn and woven fabrics of paper yarn"@en-AU ;
    skos:narrower C2004A04997:198 ;
    skos:prefLabel "Chapter C244"@en-AU ;
    dcat:accessURL <https://www.legislation.gov.au/C2004A04997/2024-07-01/2024-07-01/text/1/epub/OEBPS/document_3/document_3.html#_Toc171751574> ;
    dcat:landingPage "https://www.legislation.gov.au/C2004A04997/2024-07-01/2024-07-01/text/1/epub/OEBPS/document_3/document_3.html#_Toc171751574"^^xsd:anyURI ;
    dcat:theme legcons:Chapter .

C2004A04997:245 a legcons:Chapter,
        C2004A04997:Chapter,
        owl:Class,
        dcat:Resource ;
    rdfs:label "Chapter - C245 Chapter 54 Man made filaments strip and the like of man made textile materials"@en-AU ;
    dct:isPartOf C2004A04997:198 ;
    rdfs:comment "Chapter 54 Man made filaments strip and the like of man made textile materials - Abrievated Graph Key: C245"@en-AU ;
    rdfs:subClassOf C2004A04997: ;
    skos:definition "Chapter 54 Man made filaments strip and the like of man made textile materials"@en-AU ;
    skos:narrower C2004A04997:198 ;
    skos:prefLabel "Chapter C245"@en-AU ;
    dcat:accessURL <https://www.legislation.gov.au/C2004A04997/2024-07-01/2024-07-01/text/1/epub/OEBPS/document_3/document_3.html#_Toc171751575> ;
    dcat:landingPage "https://www.legislation.gov.au/C2004A04997/2024-07-01/2024-07-01/text/1/epub/OEBPS/document_3/document_3.html#_Toc171751575"^^xsd:anyURI ;
    dcat:theme legcons:Chapter .

C2004A04997:246 a legcons:Item,
        C2004A04997:Item,
        owl:Class,
        dcat:Resource ;
    rdfs:label "Item - I246 Notes"@en-AU ;
    dct:isPartOf C2004A04997:198 ;
    rdfs:comment "Notes - Abrievated Graph Key: I246"@en-AU ;
    rdfs:subClassOf C2004A04997: ;
    skos:definition "Notes"@en-AU ;
    skos:narrower C2004A04997:198 ;
    skos:prefLabel "Item I246"@en-AU ;
    dcat:accessURL <https://www.legislation.gov.au/C2004A04997/2024-07-01/2024-07-01/text/1/epub/OEBPS/document_3/document_3.html#_Toc171751576> ;
    dcat:landingPage "https://www.legislation.gov.au/C2004A04997/2024-07-01/2024-07-01/text/1/epub/OEBPS/document_3/document_3.html#_Toc171751576"^^xsd:anyURI ;
    dcat:theme legcons:Item .

C2004A04997:247 a legcons:Chapter,
        C2004A04997:Chapter,
        owl:Class,
        dcat:Resource ;
    rdfs:label "Chapter - C247 Chapter 55 Man made staple fibres"@en-AU ;
    dct:isPartOf C2004A04997:198 ;
    rdfs:comment "Chapter 55 Man made staple fibres - Abrievated Graph Key: C247"@en-AU ;
    rdfs:subClassOf C2004A04997: ;
    skos:definition "Chapter 55 Man made staple fibres"@en-AU ;
    skos:narrower C2004A04997:198 ;
    skos:prefLabel "Chapter C247"@en-AU ;
    dcat:accessURL <https://www.legislation.gov.au/C2004A04997/2024-07-01/2024-07-01/text/1/epub/OEBPS/document_3/document_3.html#_Toc171751577> ;
    dcat:landingPage "https://www.legislation.gov.au/C2004A04997/2024-07-01/2024-07-01/text/1/epub/OEBPS/document_3/document_3.html#_Toc171751577"^^xsd:anyURI ;
    dcat:theme legcons:Chapter .

C2004A04997:248 a legcons:Item,
        C2004A04997:Item,
        owl:Class,
        dcat:Resource ;
    rdfs:label "Item - I248 Note"@en-AU ;
    dct:isPartOf C2004A04997:198 ;
    rdfs:comment "Note - Abrievated Graph Key: I248"@en-AU ;
    rdfs:subClassOf C2004A04997: ;
    skos:definition "Note"@en-AU ;
    skos:narrower C2004A04997:198 ;
    skos:prefLabel "Item I248"@en-AU ;
    dcat:accessURL <https://www.legislation.gov.au/C2004A04997/2024-07-01/2024-07-01/text/1/epub/OEBPS/document_3/document_3.html#_Toc171751578> ;
    dcat:landingPage "https://www.legislation.gov.au/C2004A04997/2024-07-01/2024-07-01/text/1/epub/OEBPS/document_3/document_3.html#_Toc171751578"^^xsd:anyURI ;
    dcat:theme legcons:Item .

C2004A04997:249 a legcons:Chapter,
        C2004A04997:Chapter,
        owl:Class,
        dcat:Resource ;
    rdfs:label "Chapter - C249 Chapter 56 Wadding felt and nonwovens special yarns twine cordage ropes and cables and articles thereof"@en-AU ;
    dct:isPartOf C2004A04997:198 ;
    rdfs:comment "Chapter 56 Wadding felt and nonwovens special yarns twine cordage ropes and cables and articles thereof - Abrievated Graph Key: C249"@en-AU ;
    rdfs:subClassOf C2004A04997: ;
    skos:definition "Chapter 56 Wadding felt and nonwovens special yarns twine cordage ropes and cables and articles thereof"@en-AU ;
    skos:narrower C2004A04997:198 ;
    skos:prefLabel "Chapter C249"@en-AU ;
    dcat:accessURL <https://www.legislation.gov.au/C2004A04997/2024-07-01/2024-07-01/text/1/epub/OEBPS/document_3/document_3.html#_Toc171751579> ;
    dcat:landingPage "https://www.legislation.gov.au/C2004A04997/2024-07-01/2024-07-01/text/1/epub/OEBPS/document_3/document_3.html#_Toc171751579"^^xsd:anyURI ;
    dcat:theme legcons:Chapter .

C2004A04997:25 a legcons:Item,
        C2004A04997:Item,
        owl:Class,
        dcat:Resource ;
    rdfs:label "Item - I25 13 EB  When goods are Trans Pacific Partnership originating goods"@en-AU ;
    dct:isPartOf C2004A04997:2 ;
    rdfs:comment "13 EB  When goods are Trans Pacific Partnership originating goods - Abrievated Graph Key: I25"@en-AU ;
    rdfs:subClassOf C2004A04997: ;
    skos:definition "13 EB  When goods are Trans Pacific Partnership originating goods"@en-AU ;
    skos:narrower C2004A04997:2 ;
    skos:prefLabel "Item I25"@en-AU ;
    dcat:accessURL <https://www.legislation.gov.au/C2004A04997/2024-07-01/2024-07-01/text/1/epub/OEBPS/document_1/document_1.html#_Toc172806525> ;
    dcat:landingPage "https://www.legislation.gov.au/C2004A04997/2024-07-01/2024-07-01/text/1/epub/OEBPS/document_1/document_1.html#_Toc172806525"^^xsd:anyURI ;
    dcat:theme legcons:Item .

C2004A04997:250 a legcons:Item,
        C2004A04997:Item,
        owl:Class,
        dcat:Resource ;
    rdfs:label "Item - I250 Notes"@en-AU ;
    dct:isPartOf C2004A04997:198 ;
    rdfs:comment "Notes - Abrievated Graph Key: I250"@en-AU ;
    rdfs:subClassOf C2004A04997: ;
    skos:definition "Notes"@en-AU ;
    skos:narrower C2004A04997:198 ;
    skos:prefLabel "Item I250"@en-AU ;
    dcat:accessURL <https://www.legislation.gov.au/C2004A04997/2024-07-01/2024-07-01/text/1/epub/OEBPS/document_3/document_3.html#_Toc171751580> ;
    dcat:landingPage "https://www.legislation.gov.au/C2004A04997/2024-07-01/2024-07-01/text/1/epub/OEBPS/document_3/document_3.html#_Toc171751580"^^xsd:anyURI ;
    dcat:theme legcons:Item .

C2004A04997:251 a legcons:Chapter,
        C2004A04997:Chapter,
        owl:Class,
        dcat:Resource ;
    rdfs:label "Chapter - C251 Chapter 57 Carpets and other textile floor coverings"@en-AU ;
    dct:isPartOf C2004A04997:198 ;
    rdfs:comment "Chapter 57 Carpets and other textile floor coverings - Abrievated Graph Key: C251"@en-AU ;
    rdfs:subClassOf C2004A04997: ;
    skos:definition "Chapter 57 Carpets and other textile floor coverings"@en-AU ;
    skos:narrower C2004A04997:198 ;
    skos:prefLabel "Chapter C251"@en-AU ;
    dcat:accessURL <https://www.legislation.gov.au/C2004A04997/2024-07-01/2024-07-01/text/1/epub/OEBPS/document_3/document_3.html#_Toc171751581> ;
    dcat:landingPage "https://www.legislation.gov.au/C2004A04997/2024-07-01/2024-07-01/text/1/epub/OEBPS/document_3/document_3.html#_Toc171751581"^^xsd:anyURI ;
    dcat:theme legcons:Chapter .

C2004A04997:252 a legcons:Item,
        C2004A04997:Item,
        owl:Class,
        dcat:Resource ;
    rdfs:label "Item - I252 Notes"@en-AU ;
    dct:isPartOf C2004A04997:198 ;
    rdfs:comment "Notes - Abrievated Graph Key: I252"@en-AU ;
    rdfs:subClassOf C2004A04997: ;
    skos:definition "Notes"@en-AU ;
    skos:narrower C2004A04997:198 ;
    skos:prefLabel "Item I252"@en-AU ;
    dcat:accessURL <https://www.legislation.gov.au/C2004A04997/2024-07-01/2024-07-01/text/1/epub/OEBPS/document_3/document_3.html#_Toc171751582> ;
    dcat:landingPage "https://www.legislation.gov.au/C2004A04997/2024-07-01/2024-07-01/text/1/epub/OEBPS/document_3/document_3.html#_Toc171751582"^^xsd:anyURI ;
    dcat:theme legcons:Item .

C2004A04997:253 a legcons:Item,
        C2004A04997:Item,
        owl:Class,
        dcat:Resource ;
    rdfs:label "Item - I253 Additional Notes"@en-AU ;
    dct:isPartOf C2004A04997:198 ;
    rdfs:comment "Additional Notes - Abrievated Graph Key: I253"@en-AU ;
    rdfs:subClassOf C2004A04997: ;
    skos:definition "Additional Notes"@en-AU ;
    skos:narrower C2004A04997:198 ;
    skos:prefLabel "Item I253"@en-AU ;
    dcat:accessURL <https://www.legislation.gov.au/C2004A04997/2024-07-01/2024-07-01/text/1/epub/OEBPS/document_3/document_3.html#_Toc171751583> ;
    dcat:landingPage "https://www.legislation.gov.au/C2004A04997/2024-07-01/2024-07-01/text/1/epub/OEBPS/document_3/document_3.html#_Toc171751583"^^xsd:anyURI ;
    dcat:theme legcons:Item .

C2004A04997:254 a legcons:Chapter,
        C2004A04997:Chapter,
        owl:Class,
        dcat:Resource ;
    rdfs:label "Chapter - C254 Chapter 58 Special woven fabrics tufted textile fabrics lace tapestries trimmings embroidery"@en-AU ;
    dct:isPartOf C2004A04997:198 ;
    rdfs:comment "Chapter 58 Special woven fabrics tufted textile fabrics lace tapestries trimmings embroidery - Abrievated Graph Key: C254"@en-AU ;
    rdfs:subClassOf C2004A04997: ;
    skos:definition "Chapter 58 Special woven fabrics tufted textile fabrics lace tapestries trimmings embroidery"@en-AU ;
    skos:narrower C2004A04997:198 ;
    skos:prefLabel "Chapter C254"@en-AU ;
    dcat:accessURL <https://www.legislation.gov.au/C2004A04997/2024-07-01/2024-07-01/text/1/epub/OEBPS/document_3/document_3.html#_Toc171751584> ;
    dcat:landingPage "https://www.legislation.gov.au/C2004A04997/2024-07-01/2024-07-01/text/1/epub/OEBPS/document_3/document_3.html#_Toc171751584"^^xsd:anyURI ;
    dcat:theme legcons:Chapter .

C2004A04997:255 a legcons:Item,
        C2004A04997:Item,
        owl:Class,
        dcat:Resource ;
    rdfs:label "Item - I255 Notes"@en-AU ;
    dct:isPartOf C2004A04997:198 ;
    rdfs:comment "Notes - Abrievated Graph Key: I255"@en-AU ;
    rdfs:subClassOf C2004A04997: ;
    skos:definition "Notes"@en-AU ;
    skos:narrower C2004A04997:198 ;
    skos:prefLabel "Item I255"@en-AU ;
    dcat:accessURL <https://www.legislation.gov.au/C2004A04997/2024-07-01/2024-07-01/text/1/epub/OEBPS/document_3/document_3.html#_Toc171751585> ;
    dcat:landingPage "https://www.legislation.gov.au/C2004A04997/2024-07-01/2024-07-01/text/1/epub/OEBPS/document_3/document_3.html#_Toc171751585"^^xsd:anyURI ;
    dcat:theme legcons:Item .

C2004A04997:256 a legcons:Item,
        C2004A04997:Item,
        owl:Class,
        dcat:Resource ;
    rdfs:label "Item - I256 Additional Note"@en-AU ;
    dct:isPartOf C2004A04997:198 ;
    rdfs:comment "Additional Note - Abrievated Graph Key: I256"@en-AU ;
    rdfs:subClassOf C2004A04997: ;
    skos:definition "Additional Note"@en-AU ;
    skos:narrower C2004A04997:198 ;
    skos:prefLabel "Item I256"@en-AU ;
    dcat:accessURL <https://www.legislation.gov.au/C2004A04997/2024-07-01/2024-07-01/text/1/epub/OEBPS/document_3/document_3.html#_Toc171751586> ;
    dcat:landingPage "https://www.legislation.gov.au/C2004A04997/2024-07-01/2024-07-01/text/1/epub/OEBPS/document_3/document_3.html#_Toc171751586"^^xsd:anyURI ;
    dcat:theme legcons:Item .

C2004A04997:257 a legcons:Chapter,
        C2004A04997:Chapter,
        owl:Class,
        dcat:Resource ;
    rdfs:label "Chapter - C257 Chapter 59 Impregnated coated covered or laminated textile fabrics textile articles of a kind suitable for industrial use"@en-AU ;
    dct:isPartOf C2004A04997:198 ;
    rdfs:comment "Chapter 59 Impregnated coated covered or laminated textile fabrics textile articles of a kind suitable for industrial use - Abrievated Graph Key: C257"@en-AU ;
    rdfs:subClassOf C2004A04997: ;
    skos:definition "Chapter 59 Impregnated coated covered or laminated textile fabrics textile articles of a kind suitable for industrial use"@en-AU ;
    skos:narrower C2004A04997:198 ;
    skos:prefLabel "Chapter C257"@en-AU ;
    dcat:accessURL <https://www.legislation.gov.au/C2004A04997/2024-07-01/2024-07-01/text/1/epub/OEBPS/document_3/document_3.html#_Toc171751587> ;
    dcat:landingPage "https://www.legislation.gov.au/C2004A04997/2024-07-01/2024-07-01/text/1/epub/OEBPS/document_3/document_3.html#_Toc171751587"^^xsd:anyURI ;
    dcat:theme legcons:Chapter .

C2004A04997:258 a legcons:Item,
        C2004A04997:Item,
        owl:Class,
        dcat:Resource ;
    rdfs:label "Item - I258 Notes"@en-AU ;
    dct:isPartOf C2004A04997:198 ;
    rdfs:comment "Notes - Abrievated Graph Key: I258"@en-AU ;
    rdfs:subClassOf C2004A04997: ;
    skos:definition "Notes"@en-AU ;
    skos:narrower C2004A04997:198 ;
    skos:prefLabel "Item I258"@en-AU ;
    dcat:accessURL <https://www.legislation.gov.au/C2004A04997/2024-07-01/2024-07-01/text/1/epub/OEBPS/document_3/document_3.html#_Toc171751588> ;
    dcat:landingPage "https://www.legislation.gov.au/C2004A04997/2024-07-01/2024-07-01/text/1/epub/OEBPS/document_3/document_3.html#_Toc171751588"^^xsd:anyURI ;
    dcat:theme legcons:Item .

C2004A04997:26 a legcons:Item,
        C2004A04997:Item,
        owl:Class,
        dcat:Resource ;
    rdfs:label "Item - I26 13 F  When goods are Malaysian originating goods"@en-AU ;
    dct:isPartOf C2004A04997:2 ;
    rdfs:comment "13 F  When goods are Malaysian originating goods - Abrievated Graph Key: I26"@en-AU ;
    rdfs:subClassOf C2004A04997: ;
    skos:definition "13 F  When goods are Malaysian originating goods"@en-AU ;
    skos:narrower C2004A04997:2 ;
    skos:prefLabel "Item I26"@en-AU ;
    dcat:accessURL <https://www.legislation.gov.au/C2004A04997/2024-07-01/2024-07-01/text/1/epub/OEBPS/document_1/document_1.html#_Toc172806526> ;
    dcat:landingPage "https://www.legislation.gov.au/C2004A04997/2024-07-01/2024-07-01/text/1/epub/OEBPS/document_1/document_1.html#_Toc172806526"^^xsd:anyURI ;
    dcat:theme legcons:Item .

C2004A04997:260 a legcons:Schedule,
        C2004A04997:Schedule,
        owl:Class,
        dcat:Resource ;
    rdfs:label "Schedule - S260 Schedule 3 Classification of goods and general and special rates of duty"@en-AU ;
    dct:isPartOf C2004A04997:259 ;
    rdfs:comment "Schedule 3 Classification of goods and general and special rates of duty - Abrievated Graph Key: S260"@en-AU ;
    rdfs:subClassOf C2004A04997: ;
    skos:definition "Schedule 3 Classification of goods and general and special rates of duty"@en-AU ;
    skos:narrower C2004A04997:259 ;
    skos:prefLabel "Schedule S260"@en-AU ;
    dcat:accessURL <https://www.legislation.gov.au/C2004A04997/2024-07-01/2024-07-01/text/1/epub/OEBPS/document_4/document_4.html#_Toc171751991> ;
    dcat:landingPage "https://www.legislation.gov.au/C2004A04997/2024-07-01/2024-07-01/text/1/epub/OEBPS/document_4/document_4.html#_Toc171751991"^^xsd:anyURI ;
    dcat:theme legcons:Schedule .

C2004A04997:262 a legcons:Chapter,
        C2004A04997:Chapter,
        owl:Class,
        dcat:Resource ;
    rdfs:label "Chapter - C262 Chapter 60 Knitted or crocheted fabrics"@en-AU ;
    dct:isPartOf C2004A04997:261 ;
    rdfs:comment "Chapter 60 Knitted or crocheted fabrics - Abrievated Graph Key: C262"@en-AU ;
    rdfs:subClassOf C2004A04997: ;
    skos:definition "Chapter 60 Knitted or crocheted fabrics"@en-AU ;
    skos:narrower C2004A04997:261 ;
    skos:prefLabel "Chapter C262"@en-AU ;
    dcat:accessURL <https://www.legislation.gov.au/C2004A04997/2024-07-01/2024-07-01/text/1/epub/OEBPS/document_4/document_4.html#_Toc171751993> ;
    dcat:landingPage "https://www.legislation.gov.au/C2004A04997/2024-07-01/2024-07-01/text/1/epub/OEBPS/document_4/document_4.html#_Toc171751993"^^xsd:anyURI ;
    dcat:theme legcons:Chapter .

C2004A04997:263 a legcons:Item,
        C2004A04997:Item,
        owl:Class,
        dcat:Resource ;
    rdfs:label "Item - I263 Notes"@en-AU ;
    dct:isPartOf C2004A04997:261 ;
    rdfs:comment "Notes - Abrievated Graph Key: I263"@en-AU ;
    rdfs:subClassOf C2004A04997: ;
    skos:definition "Notes"@en-AU ;
    skos:narrower C2004A04997:261 ;
    skos:prefLabel "Item I263"@en-AU ;
    dcat:accessURL <https://www.legislation.gov.au/C2004A04997/2024-07-01/2024-07-01/text/1/epub/OEBPS/document_4/document_4.html#_Toc171751994> ;
    dcat:landingPage "https://www.legislation.gov.au/C2004A04997/2024-07-01/2024-07-01/text/1/epub/OEBPS/document_4/document_4.html#_Toc171751994"^^xsd:anyURI ;
    dcat:theme legcons:Item .

C2004A04997:264 a legcons:Item,
        C2004A04997:Item,
        owl:Class,
        dcat:Resource ;
    rdfs:label "Item - I264 Subheading Note"@en-AU ;
    dct:isPartOf C2004A04997:261 ;
    rdfs:comment "Subheading Note - Abrievated Graph Key: I264"@en-AU ;
    rdfs:subClassOf C2004A04997: ;
    skos:definition "Subheading Note"@en-AU ;
    skos:narrower C2004A04997:261 ;
    skos:prefLabel "Item I264"@en-AU ;
    dcat:accessURL <https://www.legislation.gov.au/C2004A04997/2024-07-01/2024-07-01/text/1/epub/OEBPS/document_4/document_4.html#_Toc171751995> ;
    dcat:landingPage "https://www.legislation.gov.au/C2004A04997/2024-07-01/2024-07-01/text/1/epub/OEBPS/document_4/document_4.html#_Toc171751995"^^xsd:anyURI ;
    dcat:theme legcons:Item .

C2004A04997:265 a legcons:Chapter,
        C2004A04997:Chapter,
        owl:Class,
        dcat:Resource ;
    rdfs:label "Chapter - C265 Chapter 61 Articles of apparel and clothing accessories knitted or crocheted"@en-AU ;
    dct:isPartOf C2004A04997:261 ;
    rdfs:comment "Chapter 61 Articles of apparel and clothing accessories knitted or crocheted - Abrievated Graph Key: C265"@en-AU ;
    rdfs:subClassOf C2004A04997: ;
    skos:definition "Chapter 61 Articles of apparel and clothing accessories knitted or crocheted"@en-AU ;
    skos:narrower C2004A04997:261 ;
    skos:prefLabel "Chapter C265"@en-AU ;
    dcat:accessURL <https://www.legislation.gov.au/C2004A04997/2024-07-01/2024-07-01/text/1/epub/OEBPS/document_4/document_4.html#_Toc171751996> ;
    dcat:landingPage "https://www.legislation.gov.au/C2004A04997/2024-07-01/2024-07-01/text/1/epub/OEBPS/document_4/document_4.html#_Toc171751996"^^xsd:anyURI ;
    dcat:theme legcons:Chapter .

C2004A04997:266 a legcons:Item,
        C2004A04997:Item,
        owl:Class,
        dcat:Resource ;
    rdfs:label "Item - I266 Notes"@en-AU ;
    dct:isPartOf C2004A04997:261 ;
    rdfs:comment "Notes - Abrievated Graph Key: I266"@en-AU ;
    rdfs:subClassOf C2004A04997: ;
    skos:definition "Notes"@en-AU ;
    skos:narrower C2004A04997:261 ;
    skos:prefLabel "Item I266"@en-AU ;
    dcat:accessURL <https://www.legislation.gov.au/C2004A04997/2024-07-01/2024-07-01/text/1/epub/OEBPS/document_4/document_4.html#_Toc171751997> ;
    dcat:landingPage "https://www.legislation.gov.au/C2004A04997/2024-07-01/2024-07-01/text/1/epub/OEBPS/document_4/document_4.html#_Toc171751997"^^xsd:anyURI ;
    dcat:theme legcons:Item .

C2004A04997:267 a legcons:Item,
        C2004A04997:Item,
        owl:Class,
        dcat:Resource ;
    rdfs:label "Item - I267 Additional Note"@en-AU ;
    dct:isPartOf C2004A04997:261 ;
    rdfs:comment "Additional Note - Abrievated Graph Key: I267"@en-AU ;
    rdfs:subClassOf C2004A04997: ;
    skos:definition "Additional Note"@en-AU ;
    skos:narrower C2004A04997:261 ;
    skos:prefLabel "Item I267"@en-AU ;
    dcat:accessURL <https://www.legislation.gov.au/C2004A04997/2024-07-01/2024-07-01/text/1/epub/OEBPS/document_4/document_4.html#_Toc171751998> ;
    dcat:landingPage "https://www.legislation.gov.au/C2004A04997/2024-07-01/2024-07-01/text/1/epub/OEBPS/document_4/document_4.html#_Toc171751998"^^xsd:anyURI ;
    dcat:theme legcons:Item .

C2004A04997:268 a legcons:Chapter,
        C2004A04997:Chapter,
        owl:Class,
        dcat:Resource ;
    rdfs:label "Chapter - C268 Chapter 62 Articles of apparel and clothing accessories not knitted or crocheted"@en-AU ;
    dct:isPartOf C2004A04997:261 ;
    rdfs:comment "Chapter 62 Articles of apparel and clothing accessories not knitted or crocheted - Abrievated Graph Key: C268"@en-AU ;
    rdfs:subClassOf C2004A04997: ;
    skos:definition "Chapter 62 Articles of apparel and clothing accessories not knitted or crocheted"@en-AU ;
    skos:narrower C2004A04997:261 ;
    skos:prefLabel "Chapter C268"@en-AU ;
    dcat:accessURL <https://www.legislation.gov.au/C2004A04997/2024-07-01/2024-07-01/text/1/epub/OEBPS/document_4/document_4.html#_Toc171751999> ;
    dcat:landingPage "https://www.legislation.gov.au/C2004A04997/2024-07-01/2024-07-01/text/1/epub/OEBPS/document_4/document_4.html#_Toc171751999"^^xsd:anyURI ;
    dcat:theme legcons:Chapter .

C2004A04997:269 a legcons:Item,
        C2004A04997:Item,
        owl:Class,
        dcat:Resource ;
    rdfs:label "Item - I269 Notes"@en-AU ;
    dct:isPartOf C2004A04997:261 ;
    rdfs:comment "Notes - Abrievated Graph Key: I269"@en-AU ;
    rdfs:subClassOf C2004A04997: ;
    skos:definition "Notes"@en-AU ;
    skos:narrower C2004A04997:261 ;
    skos:prefLabel "Item I269"@en-AU ;
    dcat:accessURL <https://www.legislation.gov.au/C2004A04997/2024-07-01/2024-07-01/text/1/epub/OEBPS/document_4/document_4.html#_Toc171752000> ;
    dcat:landingPage "https://www.legislation.gov.au/C2004A04997/2024-07-01/2024-07-01/text/1/epub/OEBPS/document_4/document_4.html#_Toc171752000"^^xsd:anyURI ;
    dcat:theme legcons:Item .

C2004A04997:27 a legcons:Item,
        C2004A04997:Item,
        owl:Class,
        dcat:Resource ;
    rdfs:label "Item - I27 13 FA  When goods are Indonesian originating goods"@en-AU ;
    dct:isPartOf C2004A04997:2 ;
    rdfs:comment "13 FA  When goods are Indonesian originating goods - Abrievated Graph Key: I27"@en-AU ;
    rdfs:subClassOf C2004A04997: ;
    skos:definition "13 FA  When goods are Indonesian originating goods"@en-AU ;
    skos:narrower C2004A04997:2 ;
    skos:prefLabel "Item I27"@en-AU ;
    dcat:accessURL <https://www.legislation.gov.au/C2004A04997/2024-07-01/2024-07-01/text/1/epub/OEBPS/document_1/document_1.html#_Toc172806527> ;
    dcat:landingPage "https://www.legislation.gov.au/C2004A04997/2024-07-01/2024-07-01/text/1/epub/OEBPS/document_1/document_1.html#_Toc172806527"^^xsd:anyURI ;
    dcat:theme legcons:Item .

C2004A04997:270 a legcons:Item,
        C2004A04997:Item,
        owl:Class,
        dcat:Resource ;
    rdfs:label "Item - I270 Additional Note"@en-AU ;
    dct:isPartOf C2004A04997:261 ;
    rdfs:comment "Additional Note - Abrievated Graph Key: I270"@en-AU ;
    rdfs:subClassOf C2004A04997: ;
    skos:definition "Additional Note"@en-AU ;
    skos:narrower C2004A04997:261 ;
    skos:prefLabel "Item I270"@en-AU ;
    dcat:accessURL <https://www.legislation.gov.au/C2004A04997/2024-07-01/2024-07-01/text/1/epub/OEBPS/document_4/document_4.html#_Toc171752001> ;
    dcat:landingPage "https://www.legislation.gov.au/C2004A04997/2024-07-01/2024-07-01/text/1/epub/OEBPS/document_4/document_4.html#_Toc171752001"^^xsd:anyURI ;
    dcat:theme legcons:Item .

C2004A04997:271 a legcons:Chapter,
        C2004A04997:Chapter,
        owl:Class,
        dcat:Resource ;
    rdfs:label "Chapter - C271 Chapter 63 Other made up textile articles sets worn clothing and worn textile articles rags"@en-AU ;
    dct:isPartOf C2004A04997:261 ;
    rdfs:comment "Chapter 63 Other made up textile articles sets worn clothing and worn textile articles rags - Abrievated Graph Key: C271"@en-AU ;
    rdfs:subClassOf C2004A04997: ;
    skos:definition "Chapter 63 Other made up textile articles sets worn clothing and worn textile articles rags"@en-AU ;
    skos:narrower C2004A04997:261 ;
    skos:prefLabel "Chapter C271"@en-AU ;
    dcat:accessURL <https://www.legislation.gov.au/C2004A04997/2024-07-01/2024-07-01/text/1/epub/OEBPS/document_4/document_4.html#_Toc171752002> ;
    dcat:landingPage "https://www.legislation.gov.au/C2004A04997/2024-07-01/2024-07-01/text/1/epub/OEBPS/document_4/document_4.html#_Toc171752002"^^xsd:anyURI ;
    dcat:theme legcons:Chapter .

C2004A04997:272 a legcons:Item,
        C2004A04997:Item,
        owl:Class,
        dcat:Resource ;
    rdfs:label "Item - I272 Notes"@en-AU ;
    dct:isPartOf C2004A04997:261 ;
    rdfs:comment "Notes - Abrievated Graph Key: I272"@en-AU ;
    rdfs:subClassOf C2004A04997: ;
    skos:definition "Notes"@en-AU ;
    skos:narrower C2004A04997:261 ;
    skos:prefLabel "Item I272"@en-AU ;
    dcat:accessURL <https://www.legislation.gov.au/C2004A04997/2024-07-01/2024-07-01/text/1/epub/OEBPS/document_4/document_4.html#_Toc171752003> ;
    dcat:landingPage "https://www.legislation.gov.au/C2004A04997/2024-07-01/2024-07-01/text/1/epub/OEBPS/document_4/document_4.html#_Toc171752003"^^xsd:anyURI ;
    dcat:theme legcons:Item .

C2004A04997:273 a legcons:Item,
        C2004A04997:Item,
        owl:Class,
        dcat:Resource ;
    rdfs:label "Item - I273 Subheading Note"@en-AU ;
    dct:isPartOf C2004A04997:261 ;
    rdfs:comment "Subheading Note - Abrievated Graph Key: I273"@en-AU ;
    rdfs:subClassOf C2004A04997: ;
    skos:definition "Subheading Note"@en-AU ;
    skos:narrower C2004A04997:261 ;
    skos:prefLabel "Item I273"@en-AU ;
    dcat:accessURL <https://www.legislation.gov.au/C2004A04997/2024-07-01/2024-07-01/text/1/epub/OEBPS/document_4/document_4.html#_Toc171752004> ;
    dcat:landingPage "https://www.legislation.gov.au/C2004A04997/2024-07-01/2024-07-01/text/1/epub/OEBPS/document_4/document_4.html#_Toc171752004"^^xsd:anyURI ;
    dcat:theme legcons:Item .

C2004A04997:274 a legcons:Item,
        C2004A04997:Item,
        owl:Class,
        dcat:Resource ;
    rdfs:label "Item - I274 Sub Chapter IOther made up textile articles"@en-AU ;
    dct:isPartOf C2004A04997:261 ;
    rdfs:comment "Sub Chapter IOther made up textile articles - Abrievated Graph Key: I274"@en-AU ;
    rdfs:subClassOf C2004A04997: ;
    skos:definition "Sub Chapter IOther made up textile articles"@en-AU ;
    skos:narrower C2004A04997:261 ;
    skos:prefLabel "Item I274"@en-AU ;
    dcat:accessURL <https://www.legislation.gov.au/C2004A04997/2024-07-01/2024-07-01/text/1/epub/OEBPS/document_4/document_4.html#_Toc171752005> ;
    dcat:landingPage "https://www.legislation.gov.au/C2004A04997/2024-07-01/2024-07-01/text/1/epub/OEBPS/document_4/document_4.html#_Toc171752005"^^xsd:anyURI ;
    dcat:theme legcons:Item .

C2004A04997:275 a legcons:Item,
        C2004A04997:Item,
        owl:Class,
        dcat:Resource ;
    rdfs:label "Item - I275 Sub Chapter IISets"@en-AU ;
    dct:isPartOf C2004A04997:261 ;
    rdfs:comment "Sub Chapter IISets - Abrievated Graph Key: I275"@en-AU ;
    rdfs:subClassOf C2004A04997: ;
    skos:definition "Sub Chapter IISets"@en-AU ;
    skos:narrower C2004A04997:261 ;
    skos:prefLabel "Item I275"@en-AU ;
    dcat:accessURL <https://www.legislation.gov.au/C2004A04997/2024-07-01/2024-07-01/text/1/epub/OEBPS/document_4/document_4.html#_Toc171752006> ;
    dcat:landingPage "https://www.legislation.gov.au/C2004A04997/2024-07-01/2024-07-01/text/1/epub/OEBPS/document_4/document_4.html#_Toc171752006"^^xsd:anyURI ;
    dcat:theme legcons:Item .

C2004A04997:276 a legcons:Item,
        C2004A04997:Item,
        owl:Class,
        dcat:Resource ;
    rdfs:label "Item - I276 Sub Chapter IIIWorn clothing and worn textile articles rags"@en-AU ;
    dct:isPartOf C2004A04997:261 ;
    rdfs:comment "Sub Chapter IIIWorn clothing and worn textile articles rags - Abrievated Graph Key: I276"@en-AU ;
    rdfs:subClassOf C2004A04997: ;
    skos:definition "Sub Chapter IIIWorn clothing and worn textile articles rags"@en-AU ;
    skos:narrower C2004A04997:261 ;
    skos:prefLabel "Item I276"@en-AU ;
    dcat:accessURL <https://www.legislation.gov.au/C2004A04997/2024-07-01/2024-07-01/text/1/epub/OEBPS/document_4/document_4.html#_Toc171752007> ;
    dcat:landingPage "https://www.legislation.gov.au/C2004A04997/2024-07-01/2024-07-01/text/1/epub/OEBPS/document_4/document_4.html#_Toc171752007"^^xsd:anyURI ;
    dcat:theme legcons:Item .

C2004A04997:279 a legcons:Item,
        C2004A04997:Item,
        owl:Class,
        dcat:Resource ;
    rdfs:label "Item - I279 Notes"@en-AU ;
    dct:isPartOf C2004A04997:278 ;
    rdfs:comment "Notes - Abrievated Graph Key: I279"@en-AU ;
    rdfs:subClassOf C2004A04997: ;
    skos:definition "Notes"@en-AU ;
    skos:narrower C2004A04997:278 ;
    skos:prefLabel "Item I279"@en-AU ;
    dcat:accessURL <https://www.legislation.gov.au/C2004A04997/2024-07-01/2024-07-01/text/1/epub/OEBPS/document_4/document_4.html#_Toc171752010> ;
    dcat:landingPage "https://www.legislation.gov.au/C2004A04997/2024-07-01/2024-07-01/text/1/epub/OEBPS/document_4/document_4.html#_Toc171752010"^^xsd:anyURI ;
    dcat:theme legcons:Item .

C2004A04997:28 a legcons:Item,
        C2004A04997:Item,
        owl:Class,
        dcat:Resource ;
    rdfs:label "Item - I28 13 G  When goods are Korean originating goods"@en-AU ;
    dct:isPartOf C2004A04997:2 ;
    rdfs:comment "13 G  When goods are Korean originating goods - Abrievated Graph Key: I28"@en-AU ;
    rdfs:subClassOf C2004A04997: ;
    skos:definition "13 G  When goods are Korean originating goods"@en-AU ;
    skos:narrower C2004A04997:2 ;
    skos:prefLabel "Item I28"@en-AU ;
    dcat:accessURL <https://www.legislation.gov.au/C2004A04997/2024-07-01/2024-07-01/text/1/epub/OEBPS/document_1/document_1.html#_Toc172806528> ;
    dcat:landingPage "https://www.legislation.gov.au/C2004A04997/2024-07-01/2024-07-01/text/1/epub/OEBPS/document_1/document_1.html#_Toc172806528"^^xsd:anyURI ;
    dcat:theme legcons:Item .

C2004A04997:280 a legcons:Item,
        C2004A04997:Item,
        owl:Class,
        dcat:Resource ;
    rdfs:label "Item - I280 Subheading Note"@en-AU ;
    dct:isPartOf C2004A04997:278 ;
    rdfs:comment "Subheading Note - Abrievated Graph Key: I280"@en-AU ;
    rdfs:subClassOf C2004A04997: ;
    skos:definition "Subheading Note"@en-AU ;
    skos:narrower C2004A04997:278 ;
    skos:prefLabel "Item I280"@en-AU ;
    dcat:accessURL <https://www.legislation.gov.au/C2004A04997/2024-07-01/2024-07-01/text/1/epub/OEBPS/document_4/document_4.html#_Toc171752011> ;
    dcat:landingPage "https://www.legislation.gov.au/C2004A04997/2024-07-01/2024-07-01/text/1/epub/OEBPS/document_4/document_4.html#_Toc171752011"^^xsd:anyURI ;
    dcat:theme legcons:Item .

C2004A04997:282 a legcons:Item,
        C2004A04997:Item,
        owl:Class,
        dcat:Resource ;
    rdfs:label "Item - I282 Notes"@en-AU ;
    dct:isPartOf C2004A04997:281 ;
    rdfs:comment "Notes - Abrievated Graph Key: I282"@en-AU ;
    rdfs:subClassOf C2004A04997: ;
    skos:definition "Notes"@en-AU ;
    skos:narrower C2004A04997:281 ;
    skos:prefLabel "Item I282"@en-AU ;
    dcat:accessURL <https://www.legislation.gov.au/C2004A04997/2024-07-01/2024-07-01/text/1/epub/OEBPS/document_4/document_4.html#_Toc171752013> ;
    dcat:landingPage "https://www.legislation.gov.au/C2004A04997/2024-07-01/2024-07-01/text/1/epub/OEBPS/document_4/document_4.html#_Toc171752013"^^xsd:anyURI ;
    dcat:theme legcons:Item .

C2004A04997:284 a legcons:Item,
        C2004A04997:Item,
        owl:Class,
        dcat:Resource ;
    rdfs:label "Item - I284 Notes"@en-AU ;
    dct:isPartOf C2004A04997:283 ;
    rdfs:comment "Notes - Abrievated Graph Key: I284"@en-AU ;
    rdfs:subClassOf C2004A04997: ;
    skos:definition "Notes"@en-AU ;
    skos:narrower C2004A04997:283 ;
    skos:prefLabel "Item I284"@en-AU ;
    dcat:accessURL <https://www.legislation.gov.au/C2004A04997/2024-07-01/2024-07-01/text/1/epub/OEBPS/document_4/document_4.html#_Toc171752015> ;
    dcat:landingPage "https://www.legislation.gov.au/C2004A04997/2024-07-01/2024-07-01/text/1/epub/OEBPS/document_4/document_4.html#_Toc171752015"^^xsd:anyURI ;
    dcat:theme legcons:Item .

C2004A04997:286 a legcons:Item,
        C2004A04997:Item,
        owl:Class,
        dcat:Resource ;
    rdfs:label "Item - I286 Notes"@en-AU ;
    dct:isPartOf C2004A04997:285 ;
    rdfs:comment "Notes - Abrievated Graph Key: I286"@en-AU ;
    rdfs:subClassOf C2004A04997: ;
    skos:definition "Notes"@en-AU ;
    skos:narrower C2004A04997:285 ;
    skos:prefLabel "Item I286"@en-AU ;
    dcat:accessURL <https://www.legislation.gov.au/C2004A04997/2024-07-01/2024-07-01/text/1/epub/OEBPS/document_4/document_4.html#_Toc171752017> ;
    dcat:landingPage "https://www.legislation.gov.au/C2004A04997/2024-07-01/2024-07-01/text/1/epub/OEBPS/document_4/document_4.html#_Toc171752017"^^xsd:anyURI ;
    dcat:theme legcons:Item .

C2004A04997:289 a legcons:Item,
        C2004A04997:Item,
        owl:Class,
        dcat:Resource ;
    rdfs:label "Item - I289 Notes"@en-AU ;
    dct:isPartOf C2004A04997:288 ;
    rdfs:comment "Notes - Abrievated Graph Key: I289"@en-AU ;
    rdfs:subClassOf C2004A04997: ;
    skos:definition "Notes"@en-AU ;
    skos:narrower C2004A04997:288 ;
    skos:prefLabel "Item I289"@en-AU ;
    dcat:accessURL <https://www.legislation.gov.au/C2004A04997/2024-07-01/2024-07-01/text/1/epub/OEBPS/document_4/document_4.html#_Toc171752020> ;
    dcat:landingPage "https://www.legislation.gov.au/C2004A04997/2024-07-01/2024-07-01/text/1/epub/OEBPS/document_4/document_4.html#_Toc171752020"^^xsd:anyURI ;
    dcat:theme legcons:Item .

C2004A04997:29 a legcons:Item,
        C2004A04997:Item,
        owl:Class,
        dcat:Resource ;
    rdfs:label "Item - I29 13 GA  When goods are Indian originating goods"@en-AU ;
    dct:isPartOf C2004A04997:2 ;
    rdfs:comment "13 GA  When goods are Indian originating goods - Abrievated Graph Key: I29"@en-AU ;
    rdfs:subClassOf C2004A04997: ;
    skos:definition "13 GA  When goods are Indian originating goods"@en-AU ;
    skos:narrower C2004A04997:2 ;
    skos:prefLabel "Item I29"@en-AU ;
    dcat:accessURL <https://www.legislation.gov.au/C2004A04997/2024-07-01/2024-07-01/text/1/epub/OEBPS/document_1/document_1.html#_Toc172806529> ;
    dcat:landingPage "https://www.legislation.gov.au/C2004A04997/2024-07-01/2024-07-01/text/1/epub/OEBPS/document_1/document_1.html#_Toc172806529"^^xsd:anyURI ;
    dcat:theme legcons:Item .

C2004A04997:291 a legcons:Item,
        C2004A04997:Item,
        owl:Class,
        dcat:Resource ;
    rdfs:label "Item - I291 Notes"@en-AU ;
    dct:isPartOf C2004A04997:290 ;
    rdfs:comment "Notes - Abrievated Graph Key: I291"@en-AU ;
    rdfs:subClassOf C2004A04997: ;
    skos:definition "Notes"@en-AU ;
    skos:narrower C2004A04997:290 ;
    skos:prefLabel "Item I291"@en-AU ;
    dcat:accessURL <https://www.legislation.gov.au/C2004A04997/2024-07-01/2024-07-01/text/1/epub/OEBPS/document_4/document_4.html#_Toc171752022> ;
    dcat:landingPage "https://www.legislation.gov.au/C2004A04997/2024-07-01/2024-07-01/text/1/epub/OEBPS/document_4/document_4.html#_Toc171752022"^^xsd:anyURI ;
    dcat:theme legcons:Item .

C2004A04997:292 a legcons:Item,
        C2004A04997:Item,
        owl:Class,
        dcat:Resource ;
    rdfs:label "Item - I292 Sub Chapter IGoods of siliceous fossil meals or of similar siliceous earths and refractory goods"@en-AU ;
    dct:isPartOf C2004A04997:290 ;
    rdfs:comment "Sub Chapter IGoods of siliceous fossil meals or of similar siliceous earths and refractory goods - Abrievated Graph Key: I292"@en-AU ;
    rdfs:subClassOf C2004A04997: ;
    skos:definition "Sub Chapter IGoods of siliceous fossil meals or of similar siliceous earths and refractory goods"@en-AU ;
    skos:narrower C2004A04997:290 ;
    skos:prefLabel "Item I292"@en-AU ;
    dcat:accessURL <https://www.legislation.gov.au/C2004A04997/2024-07-01/2024-07-01/text/1/epub/OEBPS/document_4/document_4.html#_Toc171752023> ;
    dcat:landingPage "https://www.legislation.gov.au/C2004A04997/2024-07-01/2024-07-01/text/1/epub/OEBPS/document_4/document_4.html#_Toc171752023"^^xsd:anyURI ;
    dcat:theme legcons:Item .

C2004A04997:293 a legcons:Item,
        C2004A04997:Item,
        owl:Class,
        dcat:Resource ;
    rdfs:label "Item - I293 Sub Chapter IIOther ceramic products"@en-AU ;
    dct:isPartOf C2004A04997:290 ;
    rdfs:comment "Sub Chapter IIOther ceramic products - Abrievated Graph Key: I293"@en-AU ;
    rdfs:subClassOf C2004A04997: ;
    skos:definition "Sub Chapter IIOther ceramic products"@en-AU ;
    skos:narrower C2004A04997:290 ;
    skos:prefLabel "Item I293"@en-AU ;
    dcat:accessURL <https://www.legislation.gov.au/C2004A04997/2024-07-01/2024-07-01/text/1/epub/OEBPS/document_4/document_4.html#_Toc171752024> ;
    dcat:landingPage "https://www.legislation.gov.au/C2004A04997/2024-07-01/2024-07-01/text/1/epub/OEBPS/document_4/document_4.html#_Toc171752024"^^xsd:anyURI ;
    dcat:theme legcons:Item .

C2004A04997:295 a legcons:Item,
        C2004A04997:Item,
        owl:Class,
        dcat:Resource ;
    rdfs:label "Item - I295 Notes"@en-AU ;
    dct:isPartOf C2004A04997:294 ;
    rdfs:comment "Notes - Abrievated Graph Key: I295"@en-AU ;
    rdfs:subClassOf C2004A04997: ;
    skos:definition "Notes"@en-AU ;
    skos:narrower C2004A04997:294 ;
    skos:prefLabel "Item I295"@en-AU ;
    dcat:accessURL <https://www.legislation.gov.au/C2004A04997/2024-07-01/2024-07-01/text/1/epub/OEBPS/document_4/document_4.html#_Toc171752026> ;
    dcat:landingPage "https://www.legislation.gov.au/C2004A04997/2024-07-01/2024-07-01/text/1/epub/OEBPS/document_4/document_4.html#_Toc171752026"^^xsd:anyURI ;
    dcat:theme legcons:Item .

C2004A04997:296 a legcons:Item,
        C2004A04997:Item,
        owl:Class,
        dcat:Resource ;
    rdfs:label "Item - I296 Subheading Note"@en-AU ;
    dct:isPartOf C2004A04997:294 ;
    rdfs:comment "Subheading Note - Abrievated Graph Key: I296"@en-AU ;
    rdfs:subClassOf C2004A04997: ;
    skos:definition "Subheading Note"@en-AU ;
    skos:narrower C2004A04997:294 ;
    skos:prefLabel "Item I296"@en-AU ;
    dcat:accessURL <https://www.legislation.gov.au/C2004A04997/2024-07-01/2024-07-01/text/1/epub/OEBPS/document_4/document_4.html#_Toc171752027> ;
    dcat:landingPage "https://www.legislation.gov.au/C2004A04997/2024-07-01/2024-07-01/text/1/epub/OEBPS/document_4/document_4.html#_Toc171752027"^^xsd:anyURI ;
    dcat:theme legcons:Item .

C2004A04997:299 a legcons:Item,
        C2004A04997:Item,
        owl:Class,
        dcat:Resource ;
    rdfs:label "Item - I299 Notes"@en-AU ;
    dct:isPartOf C2004A04997:298 ;
    rdfs:comment "Notes - Abrievated Graph Key: I299"@en-AU ;
    rdfs:subClassOf C2004A04997: ;
    skos:definition "Notes"@en-AU ;
    skos:narrower C2004A04997:298 ;
    skos:prefLabel "Item I299"@en-AU ;
    dcat:accessURL <https://www.legislation.gov.au/C2004A04997/2024-07-01/2024-07-01/text/1/epub/OEBPS/document_4/document_4.html#_Toc171752030> ;
    dcat:landingPage "https://www.legislation.gov.au/C2004A04997/2024-07-01/2024-07-01/text/1/epub/OEBPS/document_4/document_4.html#_Toc171752030"^^xsd:anyURI ;
    dcat:theme legcons:Item .

C2004A04997:3 a legcons:Item,
        C2004A04997:Item,
        owl:Class,
        dcat:Resource ;
    rdfs:label "Item - I3 1  Short title"@en-AU ;
    dct:isPartOf C2004A04997:2 ;
    rdfs:comment "1  Short title - Abrievated Graph Key: I3"@en-AU ;
    rdfs:subClassOf C2004A04997: ;
    skos:definition "1  Short title"@en-AU ;
    skos:narrower C2004A04997:2 ;
    skos:prefLabel "Item I3"@en-AU ;
    dcat:accessURL <https://www.legislation.gov.au/C2004A04997/2024-07-01/2024-07-01/text/1/epub/OEBPS/document_1/document_1.html#_Toc172806503> ;
    dcat:landingPage "https://www.legislation.gov.au/C2004A04997/2024-07-01/2024-07-01/text/1/epub/OEBPS/document_1/document_1.html#_Toc172806503"^^xsd:anyURI ;
    dcat:theme legcons:Item .

C2004A04997:30 a legcons:Item,
        C2004A04997:Item,
        owl:Class,
        dcat:Resource ;
    rdfs:label "Item - I30 13 H  When goods are Japanese originating goods"@en-AU ;
    dct:isPartOf C2004A04997:2 ;
    rdfs:comment "13 H  When goods are Japanese originating goods - Abrievated Graph Key: I30"@en-AU ;
    rdfs:subClassOf C2004A04997: ;
    skos:definition "13 H  When goods are Japanese originating goods"@en-AU ;
    skos:narrower C2004A04997:2 ;
    skos:prefLabel "Item I30"@en-AU ;
    dcat:accessURL <https://www.legislation.gov.au/C2004A04997/2024-07-01/2024-07-01/text/1/epub/OEBPS/document_1/document_1.html#_Toc172806530> ;
    dcat:landingPage "https://www.legislation.gov.au/C2004A04997/2024-07-01/2024-07-01/text/1/epub/OEBPS/document_1/document_1.html#_Toc172806530"^^xsd:anyURI ;
    dcat:theme legcons:Item .

C2004A04997:300 a legcons:Item,
        C2004A04997:Item,
        owl:Class,
        dcat:Resource ;
    rdfs:label "Item - I300 Subheading Notes"@en-AU ;
    dct:isPartOf C2004A04997:298 ;
    rdfs:comment "Subheading Notes - Abrievated Graph Key: I300"@en-AU ;
    rdfs:subClassOf C2004A04997: ;
    skos:definition "Subheading Notes"@en-AU ;
    skos:narrower C2004A04997:298 ;
    skos:prefLabel "Item I300"@en-AU ;
    dcat:accessURL <https://www.legislation.gov.au/C2004A04997/2024-07-01/2024-07-01/text/1/epub/OEBPS/document_4/document_4.html#_Toc171752031> ;
    dcat:landingPage "https://www.legislation.gov.au/C2004A04997/2024-07-01/2024-07-01/text/1/epub/OEBPS/document_4/document_4.html#_Toc171752031"^^xsd:anyURI ;
    dcat:theme legcons:Item .

C2004A04997:301 a legcons:Item,
        C2004A04997:Item,
        owl:Class,
        dcat:Resource ;
    rdfs:label "Item - I301 Sub Chapter INatural or cultured pearls and precious or semi precious stones"@en-AU ;
    dct:isPartOf C2004A04997:298 ;
    rdfs:comment "Sub Chapter INatural or cultured pearls and precious or semi precious stones - Abrievated Graph Key: I301"@en-AU ;
    rdfs:subClassOf C2004A04997: ;
    skos:definition "Sub Chapter INatural or cultured pearls and precious or semi precious stones"@en-AU ;
    skos:narrower C2004A04997:298 ;
    skos:prefLabel "Item I301"@en-AU ;
    dcat:accessURL <https://www.legislation.gov.au/C2004A04997/2024-07-01/2024-07-01/text/1/epub/OEBPS/document_4/document_4.html#_Toc171752032> ;
    dcat:landingPage "https://www.legislation.gov.au/C2004A04997/2024-07-01/2024-07-01/text/1/epub/OEBPS/document_4/document_4.html#_Toc171752032"^^xsd:anyURI ;
    dcat:theme legcons:Item .

C2004A04997:302 a legcons:Item,
        C2004A04997:Item,
        owl:Class,
        dcat:Resource ;
    rdfs:label "Item - I302 Sub Chapter IIPrecious metals and metals clad with precious metal"@en-AU ;
    dct:isPartOf C2004A04997:298 ;
    rdfs:comment "Sub Chapter IIPrecious metals and metals clad with precious metal - Abrievated Graph Key: I302"@en-AU ;
    rdfs:subClassOf C2004A04997: ;
    skos:definition "Sub Chapter IIPrecious metals and metals clad with precious metal"@en-AU ;
    skos:narrower C2004A04997:298 ;
    skos:prefLabel "Item I302"@en-AU ;
    dcat:accessURL <https://www.legislation.gov.au/C2004A04997/2024-07-01/2024-07-01/text/1/epub/OEBPS/document_4/document_4.html#_Toc171752033> ;
    dcat:landingPage "https://www.legislation.gov.au/C2004A04997/2024-07-01/2024-07-01/text/1/epub/OEBPS/document_4/document_4.html#_Toc171752033"^^xsd:anyURI ;
    dcat:theme legcons:Item .

C2004A04997:303 a legcons:Item,
        C2004A04997:Item,
        owl:Class,
        dcat:Resource ;
    rdfs:label "Item - I303 Sub Chapter IIIJewellery goldsmiths and silversmiths wares and other articles"@en-AU ;
    dct:isPartOf C2004A04997:298 ;
    rdfs:comment "Sub Chapter IIIJewellery goldsmiths and silversmiths wares and other articles - Abrievated Graph Key: I303"@en-AU ;
    rdfs:subClassOf C2004A04997: ;
    skos:definition "Sub Chapter IIIJewellery goldsmiths and silversmiths wares and other articles"@en-AU ;
    skos:narrower C2004A04997:298 ;
    skos:prefLabel "Item I303"@en-AU ;
    dcat:accessURL <https://www.legislation.gov.au/C2004A04997/2024-07-01/2024-07-01/text/1/epub/OEBPS/document_4/document_4.html#_Toc171752034> ;
    dcat:landingPage "https://www.legislation.gov.au/C2004A04997/2024-07-01/2024-07-01/text/1/epub/OEBPS/document_4/document_4.html#_Toc171752034"^^xsd:anyURI ;
    dcat:theme legcons:Item .

C2004A04997:305 a legcons:Item,
        C2004A04997:Item,
        owl:Class,
        dcat:Resource ;
    rdfs:label "Item - I305 Notes"@en-AU ;
    dct:isPartOf C2004A04997:304 ;
    rdfs:comment "Notes - Abrievated Graph Key: I305"@en-AU ;
    rdfs:subClassOf C2004A04997: ;
    skos:definition "Notes"@en-AU ;
    skos:narrower C2004A04997:304 ;
    skos:prefLabel "Item I305"@en-AU ;
    dcat:accessURL <https://www.legislation.gov.au/C2004A04997/2024-07-01/2024-07-01/text/1/epub/OEBPS/document_4/document_4.html#_Toc171752036> ;
    dcat:landingPage "https://www.legislation.gov.au/C2004A04997/2024-07-01/2024-07-01/text/1/epub/OEBPS/document_4/document_4.html#_Toc171752036"^^xsd:anyURI ;
    dcat:theme legcons:Item .

C2004A04997:307 a legcons:Item,
        C2004A04997:Item,
        owl:Class,
        dcat:Resource ;
    rdfs:label "Item - I307 Notes"@en-AU ;
    dct:isPartOf C2004A04997:306 ;
    rdfs:comment "Notes - Abrievated Graph Key: I307"@en-AU ;
    rdfs:subClassOf C2004A04997: ;
    skos:definition "Notes"@en-AU ;
    skos:narrower C2004A04997:306 ;
    skos:prefLabel "Item I307"@en-AU ;
    dcat:accessURL <https://www.legislation.gov.au/C2004A04997/2024-07-01/2024-07-01/text/1/epub/OEBPS/document_4/document_4.html#_Toc171752038> ;
    dcat:landingPage "https://www.legislation.gov.au/C2004A04997/2024-07-01/2024-07-01/text/1/epub/OEBPS/document_4/document_4.html#_Toc171752038"^^xsd:anyURI ;
    dcat:theme legcons:Item .

C2004A04997:308 a legcons:Item,
        C2004A04997:Item,
        owl:Class,
        dcat:Resource ;
    rdfs:label "Item - I308 Subheading Notes"@en-AU ;
    dct:isPartOf C2004A04997:306 ;
    rdfs:comment "Subheading Notes - Abrievated Graph Key: I308"@en-AU ;
    rdfs:subClassOf C2004A04997: ;
    skos:definition "Subheading Notes"@en-AU ;
    skos:narrower C2004A04997:306 ;
    skos:prefLabel "Item I308"@en-AU ;
    dcat:accessURL <https://www.legislation.gov.au/C2004A04997/2024-07-01/2024-07-01/text/1/epub/OEBPS/document_4/document_4.html#_Toc171752039> ;
    dcat:landingPage "https://www.legislation.gov.au/C2004A04997/2024-07-01/2024-07-01/text/1/epub/OEBPS/document_4/document_4.html#_Toc171752039"^^xsd:anyURI ;
    dcat:theme legcons:Item .

C2004A04997:309 a legcons:Item,
        C2004A04997:Item,
        owl:Class,
        dcat:Resource ;
    rdfs:label "Item - I309 Additional Note"@en-AU ;
    dct:isPartOf C2004A04997:306 ;
    rdfs:comment "Additional Note - Abrievated Graph Key: I309"@en-AU ;
    rdfs:subClassOf C2004A04997: ;
    skos:definition "Additional Note"@en-AU ;
    skos:narrower C2004A04997:306 ;
    skos:prefLabel "Item I309"@en-AU ;
    dcat:accessURL <https://www.legislation.gov.au/C2004A04997/2024-07-01/2024-07-01/text/1/epub/OEBPS/document_4/document_4.html#_Toc171752040> ;
    dcat:landingPage "https://www.legislation.gov.au/C2004A04997/2024-07-01/2024-07-01/text/1/epub/OEBPS/document_4/document_4.html#_Toc171752040"^^xsd:anyURI ;
    dcat:theme legcons:Item .

C2004A04997:31 a legcons:Item,
        C2004A04997:Item,
        owl:Class,
        dcat:Resource ;
    rdfs:label "Item - I31 13 J  When goods are Chinese originating goods"@en-AU ;
    dct:isPartOf C2004A04997:2 ;
    rdfs:comment "13 J  When goods are Chinese originating goods - Abrievated Graph Key: I31"@en-AU ;
    rdfs:subClassOf C2004A04997: ;
    skos:definition "13 J  When goods are Chinese originating goods"@en-AU ;
    skos:narrower C2004A04997:2 ;
    skos:prefLabel "Item I31"@en-AU ;
    dcat:accessURL <https://www.legislation.gov.au/C2004A04997/2024-07-01/2024-07-01/text/1/epub/OEBPS/document_1/document_1.html#_Toc172806531> ;
    dcat:landingPage "https://www.legislation.gov.au/C2004A04997/2024-07-01/2024-07-01/text/1/epub/OEBPS/document_1/document_1.html#_Toc172806531"^^xsd:anyURI ;
    dcat:theme legcons:Item .

C2004A04997:310 a legcons:Item,
        C2004A04997:Item,
        owl:Class,
        dcat:Resource ;
    rdfs:label "Item - I310 Sub Chapter IPrimary materials products in granular or powder form"@en-AU ;
    dct:isPartOf C2004A04997:306 ;
    rdfs:comment "Sub Chapter IPrimary materials products in granular or powder form - Abrievated Graph Key: I310"@en-AU ;
    rdfs:subClassOf C2004A04997: ;
    skos:definition "Sub Chapter IPrimary materials products in granular or powder form"@en-AU ;
    skos:narrower C2004A04997:306 ;
    skos:prefLabel "Item I310"@en-AU ;
    dcat:accessURL <https://www.legislation.gov.au/C2004A04997/2024-07-01/2024-07-01/text/1/epub/OEBPS/document_4/document_4.html#_Toc171752041> ;
    dcat:landingPage "https://www.legislation.gov.au/C2004A04997/2024-07-01/2024-07-01/text/1/epub/OEBPS/document_4/document_4.html#_Toc171752041"^^xsd:anyURI ;
    dcat:theme legcons:Item .

C2004A04997:311 a legcons:Item,
        C2004A04997:Item,
        owl:Class,
        dcat:Resource ;
    rdfs:label "Item - I311 Sub Chapter IIIron and non alloy steel"@en-AU ;
    dct:isPartOf C2004A04997:306 ;
    rdfs:comment "Sub Chapter IIIron and non alloy steel - Abrievated Graph Key: I311"@en-AU ;
    rdfs:subClassOf C2004A04997: ;
    skos:definition "Sub Chapter IIIron and non alloy steel"@en-AU ;
    skos:narrower C2004A04997:306 ;
    skos:prefLabel "Item I311"@en-AU ;
    dcat:accessURL <https://www.legislation.gov.au/C2004A04997/2024-07-01/2024-07-01/text/1/epub/OEBPS/document_4/document_4.html#_Toc171752042> ;
    dcat:landingPage "https://www.legislation.gov.au/C2004A04997/2024-07-01/2024-07-01/text/1/epub/OEBPS/document_4/document_4.html#_Toc171752042"^^xsd:anyURI ;
    dcat:theme legcons:Item .

C2004A04997:312 a legcons:Item,
        C2004A04997:Item,
        owl:Class,
        dcat:Resource ;
    rdfs:label "Item - I312 Sub Chapter IIIStainless steel"@en-AU ;
    dct:isPartOf C2004A04997:306 ;
    rdfs:comment "Sub Chapter IIIStainless steel - Abrievated Graph Key: I312"@en-AU ;
    rdfs:subClassOf C2004A04997: ;
    skos:definition "Sub Chapter IIIStainless steel"@en-AU ;
    skos:narrower C2004A04997:306 ;
    skos:prefLabel "Item I312"@en-AU ;
    dcat:accessURL <https://www.legislation.gov.au/C2004A04997/2024-07-01/2024-07-01/text/1/epub/OEBPS/document_4/document_4.html#_Toc171752043> ;
    dcat:landingPage "https://www.legislation.gov.au/C2004A04997/2024-07-01/2024-07-01/text/1/epub/OEBPS/document_4/document_4.html#_Toc171752043"^^xsd:anyURI ;
    dcat:theme legcons:Item .

C2004A04997:313 a legcons:Item,
        C2004A04997:Item,
        owl:Class,
        dcat:Resource ;
    rdfs:label "Item - I313 Sub Chapter IVOther alloy steel hollow drill bars and rods of alloy or non alloy steel"@en-AU ;
    dct:isPartOf C2004A04997:306 ;
    rdfs:comment "Sub Chapter IVOther alloy steel hollow drill bars and rods of alloy or non alloy steel - Abrievated Graph Key: I313"@en-AU ;
    rdfs:subClassOf C2004A04997: ;
    skos:definition "Sub Chapter IVOther alloy steel hollow drill bars and rods of alloy or non alloy steel"@en-AU ;
    skos:narrower C2004A04997:306 ;
    skos:prefLabel "Item I313"@en-AU ;
    dcat:accessURL <https://www.legislation.gov.au/C2004A04997/2024-07-01/2024-07-01/text/1/epub/OEBPS/document_4/document_4.html#_Toc171752044> ;
    dcat:landingPage "https://www.legislation.gov.au/C2004A04997/2024-07-01/2024-07-01/text/1/epub/OEBPS/document_4/document_4.html#_Toc171752044"^^xsd:anyURI ;
    dcat:theme legcons:Item .

C2004A04997:315 a legcons:Item,
        C2004A04997:Item,
        owl:Class,
        dcat:Resource ;
    rdfs:label "Item - I315 Notes"@en-AU ;
    dct:isPartOf C2004A04997:314 ;
    rdfs:comment "Notes - Abrievated Graph Key: I315"@en-AU ;
    rdfs:subClassOf C2004A04997: ;
    skos:definition "Notes"@en-AU ;
    skos:narrower C2004A04997:314 ;
    skos:prefLabel "Item I315"@en-AU ;
    dcat:accessURL <https://www.legislation.gov.au/C2004A04997/2024-07-01/2024-07-01/text/1/epub/OEBPS/document_4/document_4.html#_Toc171752046> ;
    dcat:landingPage "https://www.legislation.gov.au/C2004A04997/2024-07-01/2024-07-01/text/1/epub/OEBPS/document_4/document_4.html#_Toc171752046"^^xsd:anyURI ;
    dcat:theme legcons:Item .

C2004A04997:316 a legcons:Item,
        C2004A04997:Item,
        owl:Class,
        dcat:Resource ;
    rdfs:label "Item - I316 Additional Notes"@en-AU ;
    dct:isPartOf C2004A04997:314 ;
    rdfs:comment "Additional Notes - Abrievated Graph Key: I316"@en-AU ;
    rdfs:subClassOf C2004A04997: ;
    skos:definition "Additional Notes"@en-AU ;
    skos:narrower C2004A04997:314 ;
    skos:prefLabel "Item I316"@en-AU ;
    dcat:accessURL <https://www.legislation.gov.au/C2004A04997/2024-07-01/2024-07-01/text/1/epub/OEBPS/document_4/document_4.html#_Toc171752047> ;
    dcat:landingPage "https://www.legislation.gov.au/C2004A04997/2024-07-01/2024-07-01/text/1/epub/OEBPS/document_4/document_4.html#_Toc171752047"^^xsd:anyURI ;
    dcat:theme legcons:Item .

C2004A04997:317 a legcons:Volume,
        C2004A04997:Volume,
        owl:Class,
        dcat:Resource ;
    rdfs:label "Volume - V317 Volume 5"@en-AU ;
    dct:hasPart C2004A04997:318 ;
    rdfs:comment "Volume 5 - Abrievated Graph Key: V317"@en-AU ;
    rdfs:subClassOf C2004A04997: ;
    skos:broader C2004A04997:318 ;
    skos:definition "Volume 5"@en-AU ;
    skos:prefLabel "Volume V317"@en-AU ;
    dcat:accessURL <https://www.legislation.gov.au/C2004A04997/2024-07-01/2024-07-01/text/1/epub/OEBPS/document_5/document_5.html> ;
    dcat:landingPage "https://www.legislation.gov.au/C2004A04997/2024-07-01/2024-07-01/text/1/epub/OEBPS/document_5/document_5.html"^^xsd:anyURI ;
    dcat:theme legcons:Volume .

C2004A04997:319 a legcons:Section,
        C2004A04997:Section,
        owl:Class,
        dcat:Resource ;
    rdfs:label "Section - S319 Section XVBase metals and articles of base metal"@en-AU ;
    dct:isPartOf C2004A04997:318 ;
    rdfs:comment "Section XVBase metals and articles of base metal - Abrievated Graph Key: S319"@en-AU ;
    rdfs:subClassOf C2004A04997: ;
    skos:definition "Section XVBase metals and articles of base metal"@en-AU ;
    skos:narrower C2004A04997:318 ;
    skos:prefLabel "Section S319"@en-AU ;
    dcat:accessURL <https://www.legislation.gov.au/C2004A04997/2024-07-01/2024-07-01/text/1/epub/OEBPS/document_5/document_5.html#_Toc171753161> ;
    dcat:landingPage "https://www.legislation.gov.au/C2004A04997/2024-07-01/2024-07-01/text/1/epub/OEBPS/document_5/document_5.html#_Toc171753161"^^xsd:anyURI ;
    dcat:theme legcons:Section .

C2004A04997:32 a legcons:Item,
        C2004A04997:Item,
        owl:Class,
        dcat:Resource ;
    rdfs:label "Item - I32 13 K  When goods are Hong Kong originating goods"@en-AU ;
    dct:isPartOf C2004A04997:2 ;
    rdfs:comment "13 K  When goods are Hong Kong originating goods - Abrievated Graph Key: I32"@en-AU ;
    rdfs:subClassOf C2004A04997: ;
    skos:definition "13 K  When goods are Hong Kong originating goods"@en-AU ;
    skos:narrower C2004A04997:2 ;
    skos:prefLabel "Item I32"@en-AU ;
    dcat:accessURL <https://www.legislation.gov.au/C2004A04997/2024-07-01/2024-07-01/text/1/epub/OEBPS/document_1/document_1.html#_Toc172806532> ;
    dcat:landingPage "https://www.legislation.gov.au/C2004A04997/2024-07-01/2024-07-01/text/1/epub/OEBPS/document_1/document_1.html#_Toc172806532"^^xsd:anyURI ;
    dcat:theme legcons:Item .

C2004A04997:320 a legcons:Chapter,
        C2004A04997:Chapter,
        owl:Class,
        dcat:Resource ;
    rdfs:label "Chapter - C320 Chapter 74 Copper and articles thereof"@en-AU ;
    dct:isPartOf C2004A04997:318 ;
    rdfs:comment "Chapter 74 Copper and articles thereof - Abrievated Graph Key: C320"@en-AU ;
    rdfs:subClassOf C2004A04997: ;
    skos:definition "Chapter 74 Copper and articles thereof"@en-AU ;
    skos:narrower C2004A04997:318 ;
    skos:prefLabel "Chapter C320"@en-AU ;
    dcat:accessURL <https://www.legislation.gov.au/C2004A04997/2024-07-01/2024-07-01/text/1/epub/OEBPS/document_5/document_5.html#_Toc171753162> ;
    dcat:landingPage "https://www.legislation.gov.au/C2004A04997/2024-07-01/2024-07-01/text/1/epub/OEBPS/document_5/document_5.html#_Toc171753162"^^xsd:anyURI ;
    dcat:theme legcons:Chapter .

C2004A04997:321 a legcons:Item,
        C2004A04997:Item,
        owl:Class,
        dcat:Resource ;
    rdfs:label "Item - I321 Note"@en-AU ;
    dct:isPartOf C2004A04997:318 ;
    rdfs:comment "Note - Abrievated Graph Key: I321"@en-AU ;
    rdfs:subClassOf C2004A04997: ;
    skos:definition "Note"@en-AU ;
    skos:narrower C2004A04997:318 ;
    skos:prefLabel "Item I321"@en-AU ;
    dcat:accessURL <https://www.legislation.gov.au/C2004A04997/2024-07-01/2024-07-01/text/1/epub/OEBPS/document_5/document_5.html#_Toc171753163> ;
    dcat:landingPage "https://www.legislation.gov.au/C2004A04997/2024-07-01/2024-07-01/text/1/epub/OEBPS/document_5/document_5.html#_Toc171753163"^^xsd:anyURI ;
    dcat:theme legcons:Item .

C2004A04997:322 a legcons:Item,
        C2004A04997:Item,
        owl:Class,
        dcat:Resource ;
    rdfs:label "Item - I322 Subheading Note"@en-AU ;
    dct:isPartOf C2004A04997:318 ;
    rdfs:comment "Subheading Note - Abrievated Graph Key: I322"@en-AU ;
    rdfs:subClassOf C2004A04997: ;
    skos:definition "Subheading Note"@en-AU ;
    skos:narrower C2004A04997:318 ;
    skos:prefLabel "Item I322"@en-AU ;
    dcat:accessURL <https://www.legislation.gov.au/C2004A04997/2024-07-01/2024-07-01/text/1/epub/OEBPS/document_5/document_5.html#_Toc171753164> ;
    dcat:landingPage "https://www.legislation.gov.au/C2004A04997/2024-07-01/2024-07-01/text/1/epub/OEBPS/document_5/document_5.html#_Toc171753164"^^xsd:anyURI ;
    dcat:theme legcons:Item .

C2004A04997:323 a legcons:Chapter,
        C2004A04997:Chapter,
        owl:Class,
        dcat:Resource ;
    rdfs:label "Chapter - C323 Chapter 75 Nickel and articles thereof"@en-AU ;
    dct:isPartOf C2004A04997:318 ;
    rdfs:comment "Chapter 75 Nickel and articles thereof - Abrievated Graph Key: C323"@en-AU ;
    rdfs:subClassOf C2004A04997: ;
    skos:definition "Chapter 75 Nickel and articles thereof"@en-AU ;
    skos:narrower C2004A04997:318 ;
    skos:prefLabel "Chapter C323"@en-AU ;
    dcat:accessURL <https://www.legislation.gov.au/C2004A04997/2024-07-01/2024-07-01/text/1/epub/OEBPS/document_5/document_5.html#_Toc171753165> ;
    dcat:landingPage "https://www.legislation.gov.au/C2004A04997/2024-07-01/2024-07-01/text/1/epub/OEBPS/document_5/document_5.html#_Toc171753165"^^xsd:anyURI ;
    dcat:theme legcons:Chapter .

C2004A04997:324 a legcons:Item,
        C2004A04997:Item,
        owl:Class,
        dcat:Resource ;
    rdfs:label "Item - I324 Subheading Notes"@en-AU ;
    dct:isPartOf C2004A04997:318 ;
    rdfs:comment "Subheading Notes - Abrievated Graph Key: I324"@en-AU ;
    rdfs:subClassOf C2004A04997: ;
    skos:definition "Subheading Notes"@en-AU ;
    skos:narrower C2004A04997:318 ;
    skos:prefLabel "Item I324"@en-AU ;
    dcat:accessURL <https://www.legislation.gov.au/C2004A04997/2024-07-01/2024-07-01/text/1/epub/OEBPS/document_5/document_5.html#_Toc171753166> ;
    dcat:landingPage "https://www.legislation.gov.au/C2004A04997/2024-07-01/2024-07-01/text/1/epub/OEBPS/document_5/document_5.html#_Toc171753166"^^xsd:anyURI ;
    dcat:theme legcons:Item .

C2004A04997:325 a legcons:Chapter,
        C2004A04997:Chapter,
        owl:Class,
        dcat:Resource ;
    rdfs:label "Chapter - C325 Chapter 76 Aluminium and articles thereof"@en-AU ;
    dct:isPartOf C2004A04997:318 ;
    rdfs:comment "Chapter 76 Aluminium and articles thereof - Abrievated Graph Key: C325"@en-AU ;
    rdfs:subClassOf C2004A04997: ;
    skos:definition "Chapter 76 Aluminium and articles thereof"@en-AU ;
    skos:narrower C2004A04997:318 ;
    skos:prefLabel "Chapter C325"@en-AU ;
    dcat:accessURL <https://www.legislation.gov.au/C2004A04997/2024-07-01/2024-07-01/text/1/epub/OEBPS/document_5/document_5.html#_Toc171753167> ;
    dcat:landingPage "https://www.legislation.gov.au/C2004A04997/2024-07-01/2024-07-01/text/1/epub/OEBPS/document_5/document_5.html#_Toc171753167"^^xsd:anyURI ;
    dcat:theme legcons:Chapter .

C2004A04997:326 a legcons:Item,
        C2004A04997:Item,
        owl:Class,
        dcat:Resource ;
    rdfs:label "Item - I326 Subheading Notes"@en-AU ;
    dct:isPartOf C2004A04997:318 ;
    rdfs:comment "Subheading Notes - Abrievated Graph Key: I326"@en-AU ;
    rdfs:subClassOf C2004A04997: ;
    skos:definition "Subheading Notes"@en-AU ;
    skos:narrower C2004A04997:318 ;
    skos:prefLabel "Item I326"@en-AU ;
    dcat:accessURL <https://www.legislation.gov.au/C2004A04997/2024-07-01/2024-07-01/text/1/epub/OEBPS/document_5/document_5.html#_Toc171753168> ;
    dcat:landingPage "https://www.legislation.gov.au/C2004A04997/2024-07-01/2024-07-01/text/1/epub/OEBPS/document_5/document_5.html#_Toc171753168"^^xsd:anyURI ;
    dcat:theme legcons:Item .

C2004A04997:327 a legcons:Item,
        C2004A04997:Item,
        owl:Class,
        dcat:Resource ;
    rdfs:label "Item - I327 Additional Note"@en-AU ;
    dct:isPartOf C2004A04997:318 ;
    rdfs:comment "Additional Note - Abrievated Graph Key: I327"@en-AU ;
    rdfs:subClassOf C2004A04997: ;
    skos:definition "Additional Note"@en-AU ;
    skos:narrower C2004A04997:318 ;
    skos:prefLabel "Item I327"@en-AU ;
    dcat:accessURL <https://www.legislation.gov.au/C2004A04997/2024-07-01/2024-07-01/text/1/epub/OEBPS/document_5/document_5.html#_Toc171753169> ;
    dcat:landingPage "https://www.legislation.gov.au/C2004A04997/2024-07-01/2024-07-01/text/1/epub/OEBPS/document_5/document_5.html#_Toc171753169"^^xsd:anyURI ;
    dcat:theme legcons:Item .

C2004A04997:328 a legcons:Chapter,
        C2004A04997:Chapter,
        owl:Class,
        dcat:Resource ;
    rdfs:label "Chapter - C328 Chapter 78 Lead and articles thereof"@en-AU ;
    dct:isPartOf C2004A04997:318 ;
    rdfs:comment "Chapter 78 Lead and articles thereof - Abrievated Graph Key: C328"@en-AU ;
    rdfs:subClassOf C2004A04997: ;
    skos:definition "Chapter 78 Lead and articles thereof"@en-AU ;
    skos:narrower C2004A04997:318 ;
    skos:prefLabel "Chapter C328"@en-AU ;
    dcat:accessURL <https://www.legislation.gov.au/C2004A04997/2024-07-01/2024-07-01/text/1/epub/OEBPS/document_5/document_5.html#_Toc171753170> ;
    dcat:landingPage "https://www.legislation.gov.au/C2004A04997/2024-07-01/2024-07-01/text/1/epub/OEBPS/document_5/document_5.html#_Toc171753170"^^xsd:anyURI ;
    dcat:theme legcons:Chapter .

C2004A04997:329 a legcons:Item,
        C2004A04997:Item,
        owl:Class,
        dcat:Resource ;
    rdfs:label "Item - I329 Subheading Note"@en-AU ;
    dct:isPartOf C2004A04997:318 ;
    rdfs:comment "Subheading Note - Abrievated Graph Key: I329"@en-AU ;
    rdfs:subClassOf C2004A04997: ;
    skos:definition "Subheading Note"@en-AU ;
    skos:narrower C2004A04997:318 ;
    skos:prefLabel "Item I329"@en-AU ;
    dcat:accessURL <https://www.legislation.gov.au/C2004A04997/2024-07-01/2024-07-01/text/1/epub/OEBPS/document_5/document_5.html#_Toc171753171> ;
    dcat:landingPage "https://www.legislation.gov.au/C2004A04997/2024-07-01/2024-07-01/text/1/epub/OEBPS/document_5/document_5.html#_Toc171753171"^^xsd:anyURI ;
    dcat:theme legcons:Item .

C2004A04997:33 a legcons:Item,
        C2004A04997:Item,
        owl:Class,
        dcat:Resource ;
    rdfs:label "Item - I33 13 L  When goods are Regional Comprehensive Economic Partnership RCEP originating goods"@en-AU ;
    dct:isPartOf C2004A04997:2 ;
    rdfs:comment "13 L  When goods are Regional Comprehensive Economic Partnership RCEP originating goods - Abrievated Graph Key: I33"@en-AU ;
    rdfs:subClassOf C2004A04997: ;
    skos:definition "13 L  When goods are Regional Comprehensive Economic Partnership RCEP originating goods"@en-AU ;
    skos:narrower C2004A04997:2 ;
    skos:prefLabel "Item I33"@en-AU ;
    dcat:accessURL <https://www.legislation.gov.au/C2004A04997/2024-07-01/2024-07-01/text/1/epub/OEBPS/document_1/document_1.html#_Toc172806533> ;
    dcat:landingPage "https://www.legislation.gov.au/C2004A04997/2024-07-01/2024-07-01/text/1/epub/OEBPS/document_1/document_1.html#_Toc172806533"^^xsd:anyURI ;
    dcat:theme legcons:Item .

C2004A04997:330 a legcons:Chapter,
        C2004A04997:Chapter,
        owl:Class,
        dcat:Resource ;
    rdfs:label "Chapter - C330 Chapter 79 Zinc and articles thereof"@en-AU ;
    dct:isPartOf C2004A04997:318 ;
    rdfs:comment "Chapter 79 Zinc and articles thereof - Abrievated Graph Key: C330"@en-AU ;
    rdfs:subClassOf C2004A04997: ;
    skos:definition "Chapter 79 Zinc and articles thereof"@en-AU ;
    skos:narrower C2004A04997:318 ;
    skos:prefLabel "Chapter C330"@en-AU ;
    dcat:accessURL <https://www.legislation.gov.au/C2004A04997/2024-07-01/2024-07-01/text/1/epub/OEBPS/document_5/document_5.html#_Toc171753172> ;
    dcat:landingPage "https://www.legislation.gov.au/C2004A04997/2024-07-01/2024-07-01/text/1/epub/OEBPS/document_5/document_5.html#_Toc171753172"^^xsd:anyURI ;
    dcat:theme legcons:Chapter .

C2004A04997:331 a legcons:Item,
        C2004A04997:Item,
        owl:Class,
        dcat:Resource ;
    rdfs:label "Item - I331 Subheading Note"@en-AU ;
    dct:isPartOf C2004A04997:318 ;
    rdfs:comment "Subheading Note - Abrievated Graph Key: I331"@en-AU ;
    rdfs:subClassOf C2004A04997: ;
    skos:definition "Subheading Note"@en-AU ;
    skos:narrower C2004A04997:318 ;
    skos:prefLabel "Item I331"@en-AU ;
    dcat:accessURL <https://www.legislation.gov.au/C2004A04997/2024-07-01/2024-07-01/text/1/epub/OEBPS/document_5/document_5.html#_Toc171753173> ;
    dcat:landingPage "https://www.legislation.gov.au/C2004A04997/2024-07-01/2024-07-01/text/1/epub/OEBPS/document_5/document_5.html#_Toc171753173"^^xsd:anyURI ;
    dcat:theme legcons:Item .

C2004A04997:332 a legcons:Chapter,
        C2004A04997:Chapter,
        owl:Class,
        dcat:Resource ;
    rdfs:label "Chapter - C332 Chapter 80 Tin and articles thereof"@en-AU ;
    dct:isPartOf C2004A04997:318 ;
    rdfs:comment "Chapter 80 Tin and articles thereof - Abrievated Graph Key: C332"@en-AU ;
    rdfs:subClassOf C2004A04997: ;
    skos:definition "Chapter 80 Tin and articles thereof"@en-AU ;
    skos:narrower C2004A04997:318 ;
    skos:prefLabel "Chapter C332"@en-AU ;
    dcat:accessURL <https://www.legislation.gov.au/C2004A04997/2024-07-01/2024-07-01/text/1/epub/OEBPS/document_5/document_5.html#_Toc171753174> ;
    dcat:landingPage "https://www.legislation.gov.au/C2004A04997/2024-07-01/2024-07-01/text/1/epub/OEBPS/document_5/document_5.html#_Toc171753174"^^xsd:anyURI ;
    dcat:theme legcons:Chapter .

C2004A04997:333 a legcons:Item,
        C2004A04997:Item,
        owl:Class,
        dcat:Resource ;
    rdfs:label "Item - I333 Subheading Note"@en-AU ;
    dct:isPartOf C2004A04997:318 ;
    rdfs:comment "Subheading Note - Abrievated Graph Key: I333"@en-AU ;
    rdfs:subClassOf C2004A04997: ;
    skos:definition "Subheading Note"@en-AU ;
    skos:narrower C2004A04997:318 ;
    skos:prefLabel "Item I333"@en-AU ;
    dcat:accessURL <https://www.legislation.gov.au/C2004A04997/2024-07-01/2024-07-01/text/1/epub/OEBPS/document_5/document_5.html#_Toc171753175> ;
    dcat:landingPage "https://www.legislation.gov.au/C2004A04997/2024-07-01/2024-07-01/text/1/epub/OEBPS/document_5/document_5.html#_Toc171753175"^^xsd:anyURI ;
    dcat:theme legcons:Item .

C2004A04997:334 a legcons:Chapter,
        C2004A04997:Chapter,
        owl:Class,
        dcat:Resource ;
    rdfs:label "Chapter - C334 Chapter 81 Other base metals cermets articles thereof"@en-AU ;
    dct:isPartOf C2004A04997:318 ;
    rdfs:comment "Chapter 81 Other base metals cermets articles thereof - Abrievated Graph Key: C334"@en-AU ;
    rdfs:subClassOf C2004A04997: ;
    skos:definition "Chapter 81 Other base metals cermets articles thereof"@en-AU ;
    skos:narrower C2004A04997:318 ;
    skos:prefLabel "Chapter C334"@en-AU ;
    dcat:accessURL <https://www.legislation.gov.au/C2004A04997/2024-07-01/2024-07-01/text/1/epub/OEBPS/document_5/document_5.html#_Toc171753176> ;
    dcat:landingPage "https://www.legislation.gov.au/C2004A04997/2024-07-01/2024-07-01/text/1/epub/OEBPS/document_5/document_5.html#_Toc171753176"^^xsd:anyURI ;
    dcat:theme legcons:Chapter .

C2004A04997:335 a legcons:Chapter,
        C2004A04997:Chapter,
        owl:Class,
        dcat:Resource ;
    rdfs:label "Chapter - C335 Chapter 82 Tools implements cutlery spoons and forks of base metal parts thereof of base metal"@en-AU ;
    dct:isPartOf C2004A04997:318 ;
    rdfs:comment "Chapter 82 Tools implements cutlery spoons and forks of base metal parts thereof of base metal - Abrievated Graph Key: C335"@en-AU ;
    rdfs:subClassOf C2004A04997: ;
    skos:definition "Chapter 82 Tools implements cutlery spoons and forks of base metal parts thereof of base metal"@en-AU ;
    skos:narrower C2004A04997:318 ;
    skos:prefLabel "Chapter C335"@en-AU ;
    dcat:accessURL <https://www.legislation.gov.au/C2004A04997/2024-07-01/2024-07-01/text/1/epub/OEBPS/document_5/document_5.html#_Toc171753177> ;
    dcat:landingPage "https://www.legislation.gov.au/C2004A04997/2024-07-01/2024-07-01/text/1/epub/OEBPS/document_5/document_5.html#_Toc171753177"^^xsd:anyURI ;
    dcat:theme legcons:Chapter .

C2004A04997:336 a legcons:Item,
        C2004A04997:Item,
        owl:Class,
        dcat:Resource ;
    rdfs:label "Item - I336 Notes"@en-AU ;
    dct:isPartOf C2004A04997:318 ;
    rdfs:comment "Notes - Abrievated Graph Key: I336"@en-AU ;
    rdfs:subClassOf C2004A04997: ;
    skos:definition "Notes"@en-AU ;
    skos:narrower C2004A04997:318 ;
    skos:prefLabel "Item I336"@en-AU ;
    dcat:accessURL <https://www.legislation.gov.au/C2004A04997/2024-07-01/2024-07-01/text/1/epub/OEBPS/document_5/document_5.html#_Toc171753178> ;
    dcat:landingPage "https://www.legislation.gov.au/C2004A04997/2024-07-01/2024-07-01/text/1/epub/OEBPS/document_5/document_5.html#_Toc171753178"^^xsd:anyURI ;
    dcat:theme legcons:Item .

C2004A04997:337 a legcons:Chapter,
        C2004A04997:Chapter,
        owl:Class,
        dcat:Resource ;
    rdfs:label "Chapter - C337 Chapter 83 Miscellaneous articles of base metal"@en-AU ;
    dct:isPartOf C2004A04997:318 ;
    rdfs:comment "Chapter 83 Miscellaneous articles of base metal - Abrievated Graph Key: C337"@en-AU ;
    rdfs:subClassOf C2004A04997: ;
    skos:definition "Chapter 83 Miscellaneous articles of base metal"@en-AU ;
    skos:narrower C2004A04997:318 ;
    skos:prefLabel "Chapter C337"@en-AU ;
    dcat:accessURL <https://www.legislation.gov.au/C2004A04997/2024-07-01/2024-07-01/text/1/epub/OEBPS/document_5/document_5.html#_Toc171753179> ;
    dcat:landingPage "https://www.legislation.gov.au/C2004A04997/2024-07-01/2024-07-01/text/1/epub/OEBPS/document_5/document_5.html#_Toc171753179"^^xsd:anyURI ;
    dcat:theme legcons:Chapter .

C2004A04997:338 a legcons:Item,
        C2004A04997:Item,
        owl:Class,
        dcat:Resource ;
    rdfs:label "Item - I338 Notes"@en-AU ;
    dct:isPartOf C2004A04997:318 ;
    rdfs:comment "Notes - Abrievated Graph Key: I338"@en-AU ;
    rdfs:subClassOf C2004A04997: ;
    skos:definition "Notes"@en-AU ;
    skos:narrower C2004A04997:318 ;
    skos:prefLabel "Item I338"@en-AU ;
    dcat:accessURL <https://www.legislation.gov.au/C2004A04997/2024-07-01/2024-07-01/text/1/epub/OEBPS/document_5/document_5.html#_Toc171753180> ;
    dcat:landingPage "https://www.legislation.gov.au/C2004A04997/2024-07-01/2024-07-01/text/1/epub/OEBPS/document_5/document_5.html#_Toc171753180"^^xsd:anyURI ;
    dcat:theme legcons:Item .

C2004A04997:339 a legcons:Item,
        C2004A04997:Item,
        owl:Class,
        dcat:Resource ;
    rdfs:label "Item - I339 Additional Note"@en-AU ;
    dct:isPartOf C2004A04997:318 ;
    rdfs:comment "Additional Note - Abrievated Graph Key: I339"@en-AU ;
    rdfs:subClassOf C2004A04997: ;
    skos:definition "Additional Note"@en-AU ;
    skos:narrower C2004A04997:318 ;
    skos:prefLabel "Item I339"@en-AU ;
    dcat:accessURL <https://www.legislation.gov.au/C2004A04997/2024-07-01/2024-07-01/text/1/epub/OEBPS/document_5/document_5.html#_Toc171753181> ;
    dcat:landingPage "https://www.legislation.gov.au/C2004A04997/2024-07-01/2024-07-01/text/1/epub/OEBPS/document_5/document_5.html#_Toc171753181"^^xsd:anyURI ;
    dcat:theme legcons:Item .

C2004A04997:34 a legcons:Item,
        C2004A04997:Item,
        owl:Class,
        dcat:Resource ;
    rdfs:label "Item - I34 13 M  When goods are UK originating goods"@en-AU ;
    dct:isPartOf C2004A04997:2 ;
    rdfs:comment "13 M  When goods are UK originating goods - Abrievated Graph Key: I34"@en-AU ;
    rdfs:subClassOf C2004A04997: ;
    skos:definition "13 M  When goods are UK originating goods"@en-AU ;
    skos:narrower C2004A04997:2 ;
    skos:prefLabel "Item I34"@en-AU ;
    dcat:accessURL <https://www.legislation.gov.au/C2004A04997/2024-07-01/2024-07-01/text/1/epub/OEBPS/document_1/document_1.html#_Toc172806534> ;
    dcat:landingPage "https://www.legislation.gov.au/C2004A04997/2024-07-01/2024-07-01/text/1/epub/OEBPS/document_1/document_1.html#_Toc172806534"^^xsd:anyURI ;
    dcat:theme legcons:Item .

C2004A04997:340 a legcons:Section,
        C2004A04997:Section,
        owl:Class,
        dcat:Resource ;
    rdfs:label "Section - S340 Section XVIMachinery and mechanical appliances electrical equipment parts thereof sound recorders and reproducers television image and sound recorders and reproducers and parts and accessories of such articles"@en-AU ;
    dct:isPartOf C2004A04997:318 ;
    rdfs:comment "Section XVIMachinery and mechanical appliances electrical equipment parts thereof sound recorders and reproducers television image and sound recorders and reproducers and parts and accessories of such articles - Abrievated Graph Key: S340"@en-AU ;
    rdfs:subClassOf C2004A04997: ;
    skos:definition "Section XVIMachinery and mechanical appliances electrical equipment parts thereof sound recorders and reproducers television image and sound recorders and reproducers and parts and accessories of such articles"@en-AU ;
    skos:narrower C2004A04997:318 ;
    skos:prefLabel "Section S340"@en-AU ;
    dcat:accessURL <https://www.legislation.gov.au/C2004A04997/2024-07-01/2024-07-01/text/1/epub/OEBPS/document_5/document_5.html#_Toc171753182> ;
    dcat:landingPage "https://www.legislation.gov.au/C2004A04997/2024-07-01/2024-07-01/text/1/epub/OEBPS/document_5/document_5.html#_Toc171753182"^^xsd:anyURI ;
    dcat:theme legcons:Section .

C2004A04997:341 a legcons:Item,
        C2004A04997:Item,
        owl:Class,
        dcat:Resource ;
    rdfs:label "Item - I341 Notes"@en-AU ;
    dct:isPartOf C2004A04997:318 ;
    rdfs:comment "Notes - Abrievated Graph Key: I341"@en-AU ;
    rdfs:subClassOf C2004A04997: ;
    skos:definition "Notes"@en-AU ;
    skos:narrower C2004A04997:318 ;
    skos:prefLabel "Item I341"@en-AU ;
    dcat:accessURL <https://www.legislation.gov.au/C2004A04997/2024-07-01/2024-07-01/text/1/epub/OEBPS/document_5/document_5.html#_Toc171753183> ;
    dcat:landingPage "https://www.legislation.gov.au/C2004A04997/2024-07-01/2024-07-01/text/1/epub/OEBPS/document_5/document_5.html#_Toc171753183"^^xsd:anyURI ;
    dcat:theme legcons:Item .

C2004A04997:342 a legcons:Item,
        C2004A04997:Item,
        owl:Class,
        dcat:Resource ;
    rdfs:label "Item - I342 Additional Notes"@en-AU ;
    dct:isPartOf C2004A04997:318 ;
    rdfs:comment "Additional Notes - Abrievated Graph Key: I342"@en-AU ;
    rdfs:subClassOf C2004A04997: ;
    skos:definition "Additional Notes"@en-AU ;
    skos:narrower C2004A04997:318 ;
    skos:prefLabel "Item I342"@en-AU ;
    dcat:accessURL <https://www.legislation.gov.au/C2004A04997/2024-07-01/2024-07-01/text/1/epub/OEBPS/document_5/document_5.html#_Toc171753184> ;
    dcat:landingPage "https://www.legislation.gov.au/C2004A04997/2024-07-01/2024-07-01/text/1/epub/OEBPS/document_5/document_5.html#_Toc171753184"^^xsd:anyURI ;
    dcat:theme legcons:Item .

C2004A04997:343 a legcons:Chapter,
        C2004A04997:Chapter,
        owl:Class,
        dcat:Resource ;
    rdfs:label "Chapter - C343 Chapter 84 Nuclear reactors boilers machinery and mechanical appliances parts thereof"@en-AU ;
    dct:isPartOf C2004A04997:318 ;
    rdfs:comment "Chapter 84 Nuclear reactors boilers machinery and mechanical appliances parts thereof - Abrievated Graph Key: C343"@en-AU ;
    rdfs:subClassOf C2004A04997: ;
    skos:definition "Chapter 84 Nuclear reactors boilers machinery and mechanical appliances parts thereof"@en-AU ;
    skos:narrower C2004A04997:318 ;
    skos:prefLabel "Chapter C343"@en-AU ;
    dcat:accessURL <https://www.legislation.gov.au/C2004A04997/2024-07-01/2024-07-01/text/1/epub/OEBPS/document_5/document_5.html#_Toc171753185> ;
    dcat:landingPage "https://www.legislation.gov.au/C2004A04997/2024-07-01/2024-07-01/text/1/epub/OEBPS/document_5/document_5.html#_Toc171753185"^^xsd:anyURI ;
    dcat:theme legcons:Chapter .

C2004A04997:344 a legcons:Item,
        C2004A04997:Item,
        owl:Class,
        dcat:Resource ;
    rdfs:label "Item - I344 Notes"@en-AU ;
    dct:isPartOf C2004A04997:318 ;
    rdfs:comment "Notes - Abrievated Graph Key: I344"@en-AU ;
    rdfs:subClassOf C2004A04997: ;
    skos:definition "Notes"@en-AU ;
    skos:narrower C2004A04997:318 ;
    skos:prefLabel "Item I344"@en-AU ;
    dcat:accessURL <https://www.legislation.gov.au/C2004A04997/2024-07-01/2024-07-01/text/1/epub/OEBPS/document_5/document_5.html#_Toc171753186> ;
    dcat:landingPage "https://www.legislation.gov.au/C2004A04997/2024-07-01/2024-07-01/text/1/epub/OEBPS/document_5/document_5.html#_Toc171753186"^^xsd:anyURI ;
    dcat:theme legcons:Item .

C2004A04997:345 a legcons:Item,
        C2004A04997:Item,
        owl:Class,
        dcat:Resource ;
    rdfs:label "Item - I345 Subheading Notes"@en-AU ;
    dct:isPartOf C2004A04997:318 ;
    rdfs:comment "Subheading Notes - Abrievated Graph Key: I345"@en-AU ;
    rdfs:subClassOf C2004A04997: ;
    skos:definition "Subheading Notes"@en-AU ;
    skos:narrower C2004A04997:318 ;
    skos:prefLabel "Item I345"@en-AU ;
    dcat:accessURL <https://www.legislation.gov.au/C2004A04997/2024-07-01/2024-07-01/text/1/epub/OEBPS/document_5/document_5.html#_Toc171753187> ;
    dcat:landingPage "https://www.legislation.gov.au/C2004A04997/2024-07-01/2024-07-01/text/1/epub/OEBPS/document_5/document_5.html#_Toc171753187"^^xsd:anyURI ;
    dcat:theme legcons:Item .

C2004A04997:346 a legcons:Item,
        C2004A04997:Item,
        owl:Class,
        dcat:Resource ;
    rdfs:label "Item - I346 Additional Notes"@en-AU ;
    dct:isPartOf C2004A04997:318 ;
    rdfs:comment "Additional Notes - Abrievated Graph Key: I346"@en-AU ;
    rdfs:subClassOf C2004A04997: ;
    skos:definition "Additional Notes"@en-AU ;
    skos:narrower C2004A04997:318 ;
    skos:prefLabel "Item I346"@en-AU ;
    dcat:accessURL <https://www.legislation.gov.au/C2004A04997/2024-07-01/2024-07-01/text/1/epub/OEBPS/document_5/document_5.html#_Toc171753188> ;
    dcat:landingPage "https://www.legislation.gov.au/C2004A04997/2024-07-01/2024-07-01/text/1/epub/OEBPS/document_5/document_5.html#_Toc171753188"^^xsd:anyURI ;
    dcat:theme legcons:Item .

C2004A04997:347 a legcons:Chapter,
        C2004A04997:Chapter,
        owl:Class,
        dcat:Resource ;
    rdfs:label "Chapter - C347 Chapter 85 Electrical machinery and equipment and parts thereof sound recorders and reproducers television image and sound recorders and reproducers and parts and accessories of such articles"@en-AU ;
    dct:isPartOf C2004A04997:318 ;
    rdfs:comment "Chapter 85 Electrical machinery and equipment and parts thereof sound recorders and reproducers television image and sound recorders and reproducers and parts and accessories of such articles - Abrievated Graph Key: C347"@en-AU ;
    rdfs:subClassOf C2004A04997: ;
    skos:definition "Chapter 85 Electrical machinery and equipment and parts thereof sound recorders and reproducers television image and sound recorders and reproducers and parts and accessories of such articles"@en-AU ;
    skos:narrower C2004A04997:318 ;
    skos:prefLabel "Chapter C347"@en-AU ;
    dcat:accessURL <https://www.legislation.gov.au/C2004A04997/2024-07-01/2024-07-01/text/1/epub/OEBPS/document_5/document_5.html#_Toc171753189> ;
    dcat:landingPage "https://www.legislation.gov.au/C2004A04997/2024-07-01/2024-07-01/text/1/epub/OEBPS/document_5/document_5.html#_Toc171753189"^^xsd:anyURI ;
    dcat:theme legcons:Chapter .

C2004A04997:348 a legcons:Item,
        C2004A04997:Item,
        owl:Class,
        dcat:Resource ;
    rdfs:label "Item - I348 Notes"@en-AU ;
    dct:isPartOf C2004A04997:318 ;
    rdfs:comment "Notes - Abrievated Graph Key: I348"@en-AU ;
    rdfs:subClassOf C2004A04997: ;
    skos:definition "Notes"@en-AU ;
    skos:narrower C2004A04997:318 ;
    skos:prefLabel "Item I348"@en-AU ;
    dcat:accessURL <https://www.legislation.gov.au/C2004A04997/2024-07-01/2024-07-01/text/1/epub/OEBPS/document_5/document_5.html#_Toc171753190> ;
    dcat:landingPage "https://www.legislation.gov.au/C2004A04997/2024-07-01/2024-07-01/text/1/epub/OEBPS/document_5/document_5.html#_Toc171753190"^^xsd:anyURI ;
    dcat:theme legcons:Item .

C2004A04997:349 a legcons:Item,
        C2004A04997:Item,
        owl:Class,
        dcat:Resource ;
    rdfs:label "Item - I349 Subheading Notes"@en-AU ;
    dct:isPartOf C2004A04997:318 ;
    rdfs:comment "Subheading Notes - Abrievated Graph Key: I349"@en-AU ;
    rdfs:subClassOf C2004A04997: ;
    skos:definition "Subheading Notes"@en-AU ;
    skos:narrower C2004A04997:318 ;
    skos:prefLabel "Item I349"@en-AU ;
    dcat:accessURL <https://www.legislation.gov.au/C2004A04997/2024-07-01/2024-07-01/text/1/epub/OEBPS/document_5/document_5.html#_Toc171753191> ;
    dcat:landingPage "https://www.legislation.gov.au/C2004A04997/2024-07-01/2024-07-01/text/1/epub/OEBPS/document_5/document_5.html#_Toc171753191"^^xsd:anyURI ;
    dcat:theme legcons:Item .

C2004A04997:35 a legcons:Item,
        C2004A04997:Item,
        owl:Class,
        dcat:Resource ;
    rdfs:label "Item - I35 14  Application of rates of duty in relation to countries and places"@en-AU ;
    dct:isPartOf C2004A04997:2 ;
    rdfs:comment "14  Application of rates of duty in relation to countries and places - Abrievated Graph Key: I35"@en-AU ;
    rdfs:subClassOf C2004A04997: ;
    skos:definition "14  Application of rates of duty in relation to countries and places"@en-AU ;
    skos:narrower C2004A04997:2 ;
    skos:prefLabel "Item I35"@en-AU ;
    dcat:accessURL <https://www.legislation.gov.au/C2004A04997/2024-07-01/2024-07-01/text/1/epub/OEBPS/document_1/document_1.html#_Toc172806535> ;
    dcat:landingPage "https://www.legislation.gov.au/C2004A04997/2024-07-01/2024-07-01/text/1/epub/OEBPS/document_1/document_1.html#_Toc172806535"^^xsd:anyURI ;
    dcat:theme legcons:Item .

C2004A04997:350 a legcons:Item,
        C2004A04997:Item,
        owl:Class,
        dcat:Resource ;
    rdfs:label "Item - I350 Additional Notes"@en-AU ;
    dct:isPartOf C2004A04997:318 ;
    rdfs:comment "Additional Notes - Abrievated Graph Key: I350"@en-AU ;
    rdfs:subClassOf C2004A04997: ;
    skos:definition "Additional Notes"@en-AU ;
    skos:narrower C2004A04997:318 ;
    skos:prefLabel "Item I350"@en-AU ;
    dcat:accessURL <https://www.legislation.gov.au/C2004A04997/2024-07-01/2024-07-01/text/1/epub/OEBPS/document_5/document_5.html#_Toc171753192> ;
    dcat:landingPage "https://www.legislation.gov.au/C2004A04997/2024-07-01/2024-07-01/text/1/epub/OEBPS/document_5/document_5.html#_Toc171753192"^^xsd:anyURI ;
    dcat:theme legcons:Item .

C2004A04997:351 a legcons:Section,
        C2004A04997:Section,
        owl:Class,
        dcat:Resource ;
    rdfs:label "Section - S351 Section XVIIVehicles aircraft vessels and associated transport equipment"@en-AU ;
    dct:isPartOf C2004A04997:318 ;
    rdfs:comment "Section XVIIVehicles aircraft vessels and associated transport equipment - Abrievated Graph Key: S351"@en-AU ;
    rdfs:subClassOf C2004A04997: ;
    skos:definition "Section XVIIVehicles aircraft vessels and associated transport equipment"@en-AU ;
    skos:narrower C2004A04997:318 ;
    skos:prefLabel "Section S351"@en-AU ;
    dcat:accessURL <https://www.legislation.gov.au/C2004A04997/2024-07-01/2024-07-01/text/1/epub/OEBPS/document_5/document_5.html#_Toc171753193> ;
    dcat:landingPage "https://www.legislation.gov.au/C2004A04997/2024-07-01/2024-07-01/text/1/epub/OEBPS/document_5/document_5.html#_Toc171753193"^^xsd:anyURI ;
    dcat:theme legcons:Section .

C2004A04997:352 a legcons:Item,
        C2004A04997:Item,
        owl:Class,
        dcat:Resource ;
    rdfs:label "Item - I352 Notes"@en-AU ;
    dct:isPartOf C2004A04997:318 ;
    rdfs:comment "Notes - Abrievated Graph Key: I352"@en-AU ;
    rdfs:subClassOf C2004A04997: ;
    skos:definition "Notes"@en-AU ;
    skos:narrower C2004A04997:318 ;
    skos:prefLabel "Item I352"@en-AU ;
    dcat:accessURL <https://www.legislation.gov.au/C2004A04997/2024-07-01/2024-07-01/text/1/epub/OEBPS/document_5/document_5.html#_Toc171753194> ;
    dcat:landingPage "https://www.legislation.gov.au/C2004A04997/2024-07-01/2024-07-01/text/1/epub/OEBPS/document_5/document_5.html#_Toc171753194"^^xsd:anyURI ;
    dcat:theme legcons:Item .

C2004A04997:353 a legcons:Chapter,
        C2004A04997:Chapter,
        owl:Class,
        dcat:Resource ;
    rdfs:label "Chapter - C353 Chapter 86 Railway or tramway locomotives rolling stock and parts thereof railway or tramway track fixtures and fittings and parts thereof mechanical including electro mechanical traffic signalling equipment of all kinds"@en-AU ;
    dct:isPartOf C2004A04997:318 ;
    rdfs:comment "Chapter 86 Railway or tramway locomotives rolling stock and parts thereof railway or tramway track fixtures and fittings and parts thereof mechanical including electro mechanical traffic signalling equipment of all kinds - Abrievated Graph Key: C353"@en-AU ;
    rdfs:subClassOf C2004A04997: ;
    skos:definition "Chapter 86 Railway or tramway locomotives rolling stock and parts thereof railway or tramway track fixtures and fittings and parts thereof mechanical including electro mechanical traffic signalling equipment of all kinds"@en-AU ;
    skos:narrower C2004A04997:318 ;
    skos:prefLabel "Chapter C353"@en-AU ;
    dcat:accessURL <https://www.legislation.gov.au/C2004A04997/2024-07-01/2024-07-01/text/1/epub/OEBPS/document_5/document_5.html#_Toc171753195> ;
    dcat:landingPage "https://www.legislation.gov.au/C2004A04997/2024-07-01/2024-07-01/text/1/epub/OEBPS/document_5/document_5.html#_Toc171753195"^^xsd:anyURI ;
    dcat:theme legcons:Chapter .

C2004A04997:354 a legcons:Item,
        C2004A04997:Item,
        owl:Class,
        dcat:Resource ;
    rdfs:label "Item - I354 Notes"@en-AU ;
    dct:isPartOf C2004A04997:318 ;
    rdfs:comment "Notes - Abrievated Graph Key: I354"@en-AU ;
    rdfs:subClassOf C2004A04997: ;
    skos:definition "Notes"@en-AU ;
    skos:narrower C2004A04997:318 ;
    skos:prefLabel "Item I354"@en-AU ;
    dcat:accessURL <https://www.legislation.gov.au/C2004A04997/2024-07-01/2024-07-01/text/1/epub/OEBPS/document_5/document_5.html#_Toc171753196> ;
    dcat:landingPage "https://www.legislation.gov.au/C2004A04997/2024-07-01/2024-07-01/text/1/epub/OEBPS/document_5/document_5.html#_Toc171753196"^^xsd:anyURI ;
    dcat:theme legcons:Item .

C2004A04997:355 a legcons:Chapter,
        C2004A04997:Chapter,
        owl:Class,
        dcat:Resource ;
    rdfs:label "Chapter - C355 Chapter 87 Vehicles other than railway or tramway rolling stock and parts and accessories thereof"@en-AU ;
    dct:isPartOf C2004A04997:318 ;
    rdfs:comment "Chapter 87 Vehicles other than railway or tramway rolling stock and parts and accessories thereof - Abrievated Graph Key: C355"@en-AU ;
    rdfs:subClassOf C2004A04997: ;
    skos:definition "Chapter 87 Vehicles other than railway or tramway rolling stock and parts and accessories thereof"@en-AU ;
    skos:narrower C2004A04997:318 ;
    skos:prefLabel "Chapter C355"@en-AU ;
    dcat:accessURL <https://www.legislation.gov.au/C2004A04997/2024-07-01/2024-07-01/text/1/epub/OEBPS/document_5/document_5.html#_Toc171753197> ;
    dcat:landingPage "https://www.legislation.gov.au/C2004A04997/2024-07-01/2024-07-01/text/1/epub/OEBPS/document_5/document_5.html#_Toc171753197"^^xsd:anyURI ;
    dcat:theme legcons:Chapter .

C2004A04997:356 a legcons:Item,
        C2004A04997:Item,
        owl:Class,
        dcat:Resource ;
    rdfs:label "Item - I356 Notes"@en-AU ;
    dct:isPartOf C2004A04997:318 ;
    rdfs:comment "Notes - Abrievated Graph Key: I356"@en-AU ;
    rdfs:subClassOf C2004A04997: ;
    skos:definition "Notes"@en-AU ;
    skos:narrower C2004A04997:318 ;
    skos:prefLabel "Item I356"@en-AU ;
    dcat:accessURL <https://www.legislation.gov.au/C2004A04997/2024-07-01/2024-07-01/text/1/epub/OEBPS/document_5/document_5.html#_Toc171753198> ;
    dcat:landingPage "https://www.legislation.gov.au/C2004A04997/2024-07-01/2024-07-01/text/1/epub/OEBPS/document_5/document_5.html#_Toc171753198"^^xsd:anyURI ;
    dcat:theme legcons:Item .

C2004A04997:357 a legcons:Item,
        C2004A04997:Item,
        owl:Class,
        dcat:Resource ;
    rdfs:label "Item - I357 Subheading Note"@en-AU ;
    dct:isPartOf C2004A04997:318 ;
    rdfs:comment "Subheading Note - Abrievated Graph Key: I357"@en-AU ;
    rdfs:subClassOf C2004A04997: ;
    skos:definition "Subheading Note"@en-AU ;
    skos:narrower C2004A04997:318 ;
    skos:prefLabel "Item I357"@en-AU ;
    dcat:accessURL <https://www.legislation.gov.au/C2004A04997/2024-07-01/2024-07-01/text/1/epub/OEBPS/document_5/document_5.html#_Toc171753199> ;
    dcat:landingPage "https://www.legislation.gov.au/C2004A04997/2024-07-01/2024-07-01/text/1/epub/OEBPS/document_5/document_5.html#_Toc171753199"^^xsd:anyURI ;
    dcat:theme legcons:Item .

C2004A04997:358 a legcons:Item,
        C2004A04997:Item,
        owl:Class,
        dcat:Resource ;
    rdfs:label "Item - I358 Additional Notes"@en-AU ;
    dct:isPartOf C2004A04997:318 ;
    rdfs:comment "Additional Notes - Abrievated Graph Key: I358"@en-AU ;
    rdfs:subClassOf C2004A04997: ;
    skos:definition "Additional Notes"@en-AU ;
    skos:narrower C2004A04997:318 ;
    skos:prefLabel "Item I358"@en-AU ;
    dcat:accessURL <https://www.legislation.gov.au/C2004A04997/2024-07-01/2024-07-01/text/1/epub/OEBPS/document_5/document_5.html#_Toc171753200> ;
    dcat:landingPage "https://www.legislation.gov.au/C2004A04997/2024-07-01/2024-07-01/text/1/epub/OEBPS/document_5/document_5.html#_Toc171753200"^^xsd:anyURI ;
    dcat:theme legcons:Item .

C2004A04997:359 a legcons:Chapter,
        C2004A04997:Chapter,
        owl:Class,
        dcat:Resource ;
    rdfs:label "Chapter - C359 Chapter 88 Aircraft spacecraft and parts thereof"@en-AU ;
    dct:isPartOf C2004A04997:318 ;
    rdfs:comment "Chapter 88 Aircraft spacecraft and parts thereof - Abrievated Graph Key: C359"@en-AU ;
    rdfs:subClassOf C2004A04997: ;
    skos:definition "Chapter 88 Aircraft spacecraft and parts thereof"@en-AU ;
    skos:narrower C2004A04997:318 ;
    skos:prefLabel "Chapter C359"@en-AU ;
    dcat:accessURL <https://www.legislation.gov.au/C2004A04997/2024-07-01/2024-07-01/text/1/epub/OEBPS/document_5/document_5.html#_Toc171753201> ;
    dcat:landingPage "https://www.legislation.gov.au/C2004A04997/2024-07-01/2024-07-01/text/1/epub/OEBPS/document_5/document_5.html#_Toc171753201"^^xsd:anyURI ;
    dcat:theme legcons:Chapter .

C2004A04997:360 a legcons:Item,
        C2004A04997:Item,
        owl:Class,
        dcat:Resource ;
    rdfs:label "Item - I360 Note"@en-AU ;
    dct:isPartOf C2004A04997:318 ;
    rdfs:comment "Note - Abrievated Graph Key: I360"@en-AU ;
    rdfs:subClassOf C2004A04997: ;
    skos:definition "Note"@en-AU ;
    skos:narrower C2004A04997:318 ;
    skos:prefLabel "Item I360"@en-AU ;
    dcat:accessURL <https://www.legislation.gov.au/C2004A04997/2024-07-01/2024-07-01/text/1/epub/OEBPS/document_5/document_5.html#_Toc171753202> ;
    dcat:landingPage "https://www.legislation.gov.au/C2004A04997/2024-07-01/2024-07-01/text/1/epub/OEBPS/document_5/document_5.html#_Toc171753202"^^xsd:anyURI ;
    dcat:theme legcons:Item .

C2004A04997:361 a legcons:Item,
        C2004A04997:Item,
        owl:Class,
        dcat:Resource ;
    rdfs:label "Item - I361 Subheading Notes"@en-AU ;
    dct:isPartOf C2004A04997:318 ;
    rdfs:comment "Subheading Notes - Abrievated Graph Key: I361"@en-AU ;
    rdfs:subClassOf C2004A04997: ;
    skos:definition "Subheading Notes"@en-AU ;
    skos:narrower C2004A04997:318 ;
    skos:prefLabel "Item I361"@en-AU ;
    dcat:accessURL <https://www.legislation.gov.au/C2004A04997/2024-07-01/2024-07-01/text/1/epub/OEBPS/document_5/document_5.html#_Toc171753203> ;
    dcat:landingPage "https://www.legislation.gov.au/C2004A04997/2024-07-01/2024-07-01/text/1/epub/OEBPS/document_5/document_5.html#_Toc171753203"^^xsd:anyURI ;
    dcat:theme legcons:Item .

C2004A04997:362 a legcons:Chapter,
        C2004A04997:Chapter,
        owl:Class,
        dcat:Resource ;
    rdfs:label "Chapter - C362 Chapter 89 Ships boats and floating structures"@en-AU ;
    dct:isPartOf C2004A04997:318 ;
    rdfs:comment "Chapter 89 Ships boats and floating structures - Abrievated Graph Key: C362"@en-AU ;
    rdfs:subClassOf C2004A04997: ;
    skos:definition "Chapter 89 Ships boats and floating structures"@en-AU ;
    skos:narrower C2004A04997:318 ;
    skos:prefLabel "Chapter C362"@en-AU ;
    dcat:accessURL <https://www.legislation.gov.au/C2004A04997/2024-07-01/2024-07-01/text/1/epub/OEBPS/document_5/document_5.html#_Toc171753204> ;
    dcat:landingPage "https://www.legislation.gov.au/C2004A04997/2024-07-01/2024-07-01/text/1/epub/OEBPS/document_5/document_5.html#_Toc171753204"^^xsd:anyURI ;
    dcat:theme legcons:Chapter .

C2004A04997:363 a legcons:Item,
        C2004A04997:Item,
        owl:Class,
        dcat:Resource ;
    rdfs:label "Item - I363 Note"@en-AU ;
    dct:isPartOf C2004A04997:318 ;
    rdfs:comment "Note - Abrievated Graph Key: I363"@en-AU ;
    rdfs:subClassOf C2004A04997: ;
    skos:definition "Note"@en-AU ;
    skos:narrower C2004A04997:318 ;
    skos:prefLabel "Item I363"@en-AU ;
    dcat:accessURL <https://www.legislation.gov.au/C2004A04997/2024-07-01/2024-07-01/text/1/epub/OEBPS/document_5/document_5.html#_Toc171753205> ;
    dcat:landingPage "https://www.legislation.gov.au/C2004A04997/2024-07-01/2024-07-01/text/1/epub/OEBPS/document_5/document_5.html#_Toc171753205"^^xsd:anyURI ;
    dcat:theme legcons:Item .

C2004A04997:364 a legcons:Section,
        C2004A04997:Section,
        owl:Class,
        dcat:Resource ;
    rdfs:label "Section - S364 Section XVIIIOptical photographic cinematographic measuring checking precision medical or surgical instruments and apparatus clocks and watches musical instruments parts and accessories thereof"@en-AU ;
    dct:isPartOf C2004A04997:318 ;
    rdfs:comment "Section XVIIIOptical photographic cinematographic measuring checking precision medical or surgical instruments and apparatus clocks and watches musical instruments parts and accessories thereof - Abrievated Graph Key: S364"@en-AU ;
    rdfs:subClassOf C2004A04997: ;
    skos:definition "Section XVIIIOptical photographic cinematographic measuring checking precision medical or surgical instruments and apparatus clocks and watches musical instruments parts and accessories thereof"@en-AU ;
    skos:narrower C2004A04997:318 ;
    skos:prefLabel "Section S364"@en-AU ;
    dcat:accessURL <https://www.legislation.gov.au/C2004A04997/2024-07-01/2024-07-01/text/1/epub/OEBPS/document_5/document_5.html#_Toc171753206> ;
    dcat:landingPage "https://www.legislation.gov.au/C2004A04997/2024-07-01/2024-07-01/text/1/epub/OEBPS/document_5/document_5.html#_Toc171753206"^^xsd:anyURI ;
    dcat:theme legcons:Section .

C2004A04997:365 a legcons:Chapter,
        C2004A04997:Chapter,
        owl:Class,
        dcat:Resource ;
    rdfs:label "Chapter - C365 Chapter 90 Optical photographic cinematographic measuring checking precision medical or surgical instruments and apparatus parts and accessories thereof"@en-AU ;
    dct:isPartOf C2004A04997:318 ;
    rdfs:comment "Chapter 90 Optical photographic cinematographic measuring checking precision medical or surgical instruments and apparatus parts and accessories thereof - Abrievated Graph Key: C365"@en-AU ;
    rdfs:subClassOf C2004A04997: ;
    skos:definition "Chapter 90 Optical photographic cinematographic measuring checking precision medical or surgical instruments and apparatus parts and accessories thereof"@en-AU ;
    skos:narrower C2004A04997:318 ;
    skos:prefLabel "Chapter C365"@en-AU ;
    dcat:accessURL <https://www.legislation.gov.au/C2004A04997/2024-07-01/2024-07-01/text/1/epub/OEBPS/document_5/document_5.html#_Toc171753207> ;
    dcat:landingPage "https://www.legislation.gov.au/C2004A04997/2024-07-01/2024-07-01/text/1/epub/OEBPS/document_5/document_5.html#_Toc171753207"^^xsd:anyURI ;
    dcat:theme legcons:Chapter .

C2004A04997:366 a legcons:Item,
        C2004A04997:Item,
        owl:Class,
        dcat:Resource ;
    rdfs:label "Item - I366 Notes"@en-AU ;
    dct:isPartOf C2004A04997:318 ;
    rdfs:comment "Notes - Abrievated Graph Key: I366"@en-AU ;
    rdfs:subClassOf C2004A04997: ;
    skos:definition "Notes"@en-AU ;
    skos:narrower C2004A04997:318 ;
    skos:prefLabel "Item I366"@en-AU ;
    dcat:accessURL <https://www.legislation.gov.au/C2004A04997/2024-07-01/2024-07-01/text/1/epub/OEBPS/document_5/document_5.html#_Toc171753208> ;
    dcat:landingPage "https://www.legislation.gov.au/C2004A04997/2024-07-01/2024-07-01/text/1/epub/OEBPS/document_5/document_5.html#_Toc171753208"^^xsd:anyURI ;
    dcat:theme legcons:Item .

C2004A04997:367 a legcons:Item,
        C2004A04997:Item,
        owl:Class,
        dcat:Resource ;
    rdfs:label "Item - I367 Additional Notes"@en-AU ;
    dct:isPartOf C2004A04997:318 ;
    rdfs:comment "Additional Notes - Abrievated Graph Key: I367"@en-AU ;
    rdfs:subClassOf C2004A04997: ;
    skos:definition "Additional Notes"@en-AU ;
    skos:narrower C2004A04997:318 ;
    skos:prefLabel "Item I367"@en-AU ;
    dcat:accessURL <https://www.legislation.gov.au/C2004A04997/2024-07-01/2024-07-01/text/1/epub/OEBPS/document_5/document_5.html#_Toc171753209> ;
    dcat:landingPage "https://www.legislation.gov.au/C2004A04997/2024-07-01/2024-07-01/text/1/epub/OEBPS/document_5/document_5.html#_Toc171753209"^^xsd:anyURI ;
    dcat:theme legcons:Item .

C2004A04997:368 a legcons:Chapter,
        C2004A04997:Chapter,
        owl:Class,
        dcat:Resource ;
    rdfs:label "Chapter - C368 Chapter 91 Clocks and watches and parts thereof"@en-AU ;
    dct:isPartOf C2004A04997:318 ;
    rdfs:comment "Chapter 91 Clocks and watches and parts thereof - Abrievated Graph Key: C368"@en-AU ;
    rdfs:subClassOf C2004A04997: ;
    skos:definition "Chapter 91 Clocks and watches and parts thereof"@en-AU ;
    skos:narrower C2004A04997:318 ;
    skos:prefLabel "Chapter C368"@en-AU ;
    dcat:accessURL <https://www.legislation.gov.au/C2004A04997/2024-07-01/2024-07-01/text/1/epub/OEBPS/document_5/document_5.html#_Toc171753210> ;
    dcat:landingPage "https://www.legislation.gov.au/C2004A04997/2024-07-01/2024-07-01/text/1/epub/OEBPS/document_5/document_5.html#_Toc171753210"^^xsd:anyURI ;
    dcat:theme legcons:Chapter .

C2004A04997:369 a legcons:Item,
        C2004A04997:Item,
        owl:Class,
        dcat:Resource ;
    rdfs:label "Item - I369 Notes"@en-AU ;
    dct:isPartOf C2004A04997:318 ;
    rdfs:comment "Notes - Abrievated Graph Key: I369"@en-AU ;
    rdfs:subClassOf C2004A04997: ;
    skos:definition "Notes"@en-AU ;
    skos:narrower C2004A04997:318 ;
    skos:prefLabel "Item I369"@en-AU ;
    dcat:accessURL <https://www.legislation.gov.au/C2004A04997/2024-07-01/2024-07-01/text/1/epub/OEBPS/document_5/document_5.html#_Toc171753211> ;
    dcat:landingPage "https://www.legislation.gov.au/C2004A04997/2024-07-01/2024-07-01/text/1/epub/OEBPS/document_5/document_5.html#_Toc171753211"^^xsd:anyURI ;
    dcat:theme legcons:Item .

C2004A04997:37 a legcons:Item,
        C2004A04997:Item,
        owl:Class,
        dcat:Resource ;
    rdfs:label "Item - I37 15  Imposition of duties"@en-AU ;
    dct:isPartOf C2004A04997:36 ;
    rdfs:comment "15  Imposition of duties - Abrievated Graph Key: I37"@en-AU ;
    rdfs:subClassOf C2004A04997: ;
    skos:definition "15  Imposition of duties"@en-AU ;
    skos:narrower C2004A04997:36 ;
    skos:prefLabel "Item I37"@en-AU ;
    dcat:accessURL <https://www.legislation.gov.au/C2004A04997/2024-07-01/2024-07-01/text/1/epub/OEBPS/document_1/document_1.html#_Toc172806537> ;
    dcat:landingPage "https://www.legislation.gov.au/C2004A04997/2024-07-01/2024-07-01/text/1/epub/OEBPS/document_1/document_1.html#_Toc172806537"^^xsd:anyURI ;
    dcat:theme legcons:Item .

C2004A04997:370 a legcons:Chapter,
        C2004A04997:Chapter,
        owl:Class,
        dcat:Resource ;
    rdfs:label "Chapter - C370 Chapter 92 Musical instruments parts and accessories of such articles"@en-AU ;
    dct:isPartOf C2004A04997:318 ;
    rdfs:comment "Chapter 92 Musical instruments parts and accessories of such articles - Abrievated Graph Key: C370"@en-AU ;
    rdfs:subClassOf C2004A04997: ;
    skos:definition "Chapter 92 Musical instruments parts and accessories of such articles"@en-AU ;
    skos:narrower C2004A04997:318 ;
    skos:prefLabel "Chapter C370"@en-AU ;
    dcat:accessURL <https://www.legislation.gov.au/C2004A04997/2024-07-01/2024-07-01/text/1/epub/OEBPS/document_5/document_5.html#_Toc171753212> ;
    dcat:landingPage "https://www.legislation.gov.au/C2004A04997/2024-07-01/2024-07-01/text/1/epub/OEBPS/document_5/document_5.html#_Toc171753212"^^xsd:anyURI ;
    dcat:theme legcons:Chapter .

C2004A04997:371 a legcons:Item,
        C2004A04997:Item,
        owl:Class,
        dcat:Resource ;
    rdfs:label "Item - I371 Notes"@en-AU ;
    dct:isPartOf C2004A04997:318 ;
    rdfs:comment "Notes - Abrievated Graph Key: I371"@en-AU ;
    rdfs:subClassOf C2004A04997: ;
    skos:definition "Notes"@en-AU ;
    skos:narrower C2004A04997:318 ;
    skos:prefLabel "Item I371"@en-AU ;
    dcat:accessURL <https://www.legislation.gov.au/C2004A04997/2024-07-01/2024-07-01/text/1/epub/OEBPS/document_5/document_5.html#_Toc171753213> ;
    dcat:landingPage "https://www.legislation.gov.au/C2004A04997/2024-07-01/2024-07-01/text/1/epub/OEBPS/document_5/document_5.html#_Toc171753213"^^xsd:anyURI ;
    dcat:theme legcons:Item .

C2004A04997:372 a legcons:Section,
        C2004A04997:Section,
        owl:Class,
        dcat:Resource ;
    rdfs:label "Section - S372 Section XIXArms and ammunition parts and accessories thereof"@en-AU ;
    dct:isPartOf C2004A04997:318 ;
    rdfs:comment "Section XIXArms and ammunition parts and accessories thereof - Abrievated Graph Key: S372"@en-AU ;
    rdfs:subClassOf C2004A04997: ;
    skos:definition "Section XIXArms and ammunition parts and accessories thereof"@en-AU ;
    skos:narrower C2004A04997:318 ;
    skos:prefLabel "Section S372"@en-AU ;
    dcat:accessURL <https://www.legislation.gov.au/C2004A04997/2024-07-01/2024-07-01/text/1/epub/OEBPS/document_5/document_5.html#_Toc171753214> ;
    dcat:landingPage "https://www.legislation.gov.au/C2004A04997/2024-07-01/2024-07-01/text/1/epub/OEBPS/document_5/document_5.html#_Toc171753214"^^xsd:anyURI ;
    dcat:theme legcons:Section .

C2004A04997:373 a legcons:Chapter,
        C2004A04997:Chapter,
        owl:Class,
        dcat:Resource ;
    rdfs:label "Chapter - C373 Chapter 93 Arms and ammunition parts and accessories thereof"@en-AU ;
    dct:isPartOf C2004A04997:318 ;
    rdfs:comment "Chapter 93 Arms and ammunition parts and accessories thereof - Abrievated Graph Key: C373"@en-AU ;
    rdfs:subClassOf C2004A04997: ;
    skos:definition "Chapter 93 Arms and ammunition parts and accessories thereof"@en-AU ;
    skos:narrower C2004A04997:318 ;
    skos:prefLabel "Chapter C373"@en-AU ;
    dcat:accessURL <https://www.legislation.gov.au/C2004A04997/2024-07-01/2024-07-01/text/1/epub/OEBPS/document_5/document_5.html#_Toc171753215> ;
    dcat:landingPage "https://www.legislation.gov.au/C2004A04997/2024-07-01/2024-07-01/text/1/epub/OEBPS/document_5/document_5.html#_Toc171753215"^^xsd:anyURI ;
    dcat:theme legcons:Chapter .

C2004A04997:374 a legcons:Item,
        C2004A04997:Item,
        owl:Class,
        dcat:Resource ;
    rdfs:label "Item - I374 Notes"@en-AU ;
    dct:isPartOf C2004A04997:318 ;
    rdfs:comment "Notes - Abrievated Graph Key: I374"@en-AU ;
    rdfs:subClassOf C2004A04997: ;
    skos:definition "Notes"@en-AU ;
    skos:narrower C2004A04997:318 ;
    skos:prefLabel "Item I374"@en-AU ;
    dcat:accessURL <https://www.legislation.gov.au/C2004A04997/2024-07-01/2024-07-01/text/1/epub/OEBPS/document_5/document_5.html#_Toc171753216> ;
    dcat:landingPage "https://www.legislation.gov.au/C2004A04997/2024-07-01/2024-07-01/text/1/epub/OEBPS/document_5/document_5.html#_Toc171753216"^^xsd:anyURI ;
    dcat:theme legcons:Item .

C2004A04997:375 a legcons:Section,
        C2004A04997:Section,
        owl:Class,
        dcat:Resource ;
    rdfs:label "Section - S375 Section XXMiscellaneous manufactured articles"@en-AU ;
    dct:isPartOf C2004A04997:318 ;
    rdfs:comment "Section XXMiscellaneous manufactured articles - Abrievated Graph Key: S375"@en-AU ;
    rdfs:subClassOf C2004A04997: ;
    skos:definition "Section XXMiscellaneous manufactured articles"@en-AU ;
    skos:narrower C2004A04997:318 ;
    skos:prefLabel "Section S375"@en-AU ;
    dcat:accessURL <https://www.legislation.gov.au/C2004A04997/2024-07-01/2024-07-01/text/1/epub/OEBPS/document_5/document_5.html#_Toc171753217> ;
    dcat:landingPage "https://www.legislation.gov.au/C2004A04997/2024-07-01/2024-07-01/text/1/epub/OEBPS/document_5/document_5.html#_Toc171753217"^^xsd:anyURI ;
    dcat:theme legcons:Section .

C2004A04997:376 a legcons:Chapter,
        C2004A04997:Chapter,
        owl:Class,
        dcat:Resource ;
    rdfs:label "Chapter - C376 Chapter 94 Furniture bedding mattresses mattress supports cushions and similar stuffed furnishings luminaires and lighting fittings not elsewhere specified or included illuminated signs illuminated name plates and the like prefabricated buildings"@en-AU ;
    dct:isPartOf C2004A04997:318 ;
    rdfs:comment "Chapter 94 Furniture bedding mattresses mattress supports cushions and similar stuffed furnishings luminaires and lighting fittings not elsewhere specified or included illuminated signs illuminated name plates and the like prefabricated buildings - Abrievated Graph Key: C376"@en-AU ;
    rdfs:subClassOf C2004A04997: ;
    skos:definition "Chapter 94 Furniture bedding mattresses mattress supports cushions and similar stuffed furnishings luminaires and lighting fittings not elsewhere specified or included illuminated signs illuminated name plates and the like prefabricated buildings"@en-AU ;
    skos:narrower C2004A04997:318 ;
    skos:prefLabel "Chapter C376"@en-AU ;
    dcat:accessURL <https://www.legislation.gov.au/C2004A04997/2024-07-01/2024-07-01/text/1/epub/OEBPS/document_5/document_5.html#_Toc171753218> ;
    dcat:landingPage "https://www.legislation.gov.au/C2004A04997/2024-07-01/2024-07-01/text/1/epub/OEBPS/document_5/document_5.html#_Toc171753218"^^xsd:anyURI ;
    dcat:theme legcons:Chapter .

C2004A04997:377 a legcons:Item,
        C2004A04997:Item,
        owl:Class,
        dcat:Resource ;
    rdfs:label "Item - I377 Notes"@en-AU ;
    dct:isPartOf C2004A04997:318 ;
    rdfs:comment "Notes - Abrievated Graph Key: I377"@en-AU ;
    rdfs:subClassOf C2004A04997: ;
    skos:definition "Notes"@en-AU ;
    skos:narrower C2004A04997:318 ;
    skos:prefLabel "Item I377"@en-AU ;
    dcat:accessURL <https://www.legislation.gov.au/C2004A04997/2024-07-01/2024-07-01/text/1/epub/OEBPS/document_5/document_5.html#_Toc171753219> ;
    dcat:landingPage "https://www.legislation.gov.au/C2004A04997/2024-07-01/2024-07-01/text/1/epub/OEBPS/document_5/document_5.html#_Toc171753219"^^xsd:anyURI ;
    dcat:theme legcons:Item .

C2004A04997:378 a legcons:Item,
        C2004A04997:Item,
        owl:Class,
        dcat:Resource ;
    rdfs:label "Item - I378 Additional Note"@en-AU ;
    dct:isPartOf C2004A04997:318 ;
    rdfs:comment "Additional Note - Abrievated Graph Key: I378"@en-AU ;
    rdfs:subClassOf C2004A04997: ;
    skos:definition "Additional Note"@en-AU ;
    skos:narrower C2004A04997:318 ;
    skos:prefLabel "Item I378"@en-AU ;
    dcat:accessURL <https://www.legislation.gov.au/C2004A04997/2024-07-01/2024-07-01/text/1/epub/OEBPS/document_5/document_5.html#_Toc171753220> ;
    dcat:landingPage "https://www.legislation.gov.au/C2004A04997/2024-07-01/2024-07-01/text/1/epub/OEBPS/document_5/document_5.html#_Toc171753220"^^xsd:anyURI ;
    dcat:theme legcons:Item .

C2004A04997:379 a legcons:Chapter,
        C2004A04997:Chapter,
        owl:Class,
        dcat:Resource ;
    rdfs:label "Chapter - C379 Chapter 95 Toys games and sports requisites parts and accessories thereof"@en-AU ;
    dct:isPartOf C2004A04997:318 ;
    rdfs:comment "Chapter 95 Toys games and sports requisites parts and accessories thereof - Abrievated Graph Key: C379"@en-AU ;
    rdfs:subClassOf C2004A04997: ;
    skos:definition "Chapter 95 Toys games and sports requisites parts and accessories thereof"@en-AU ;
    skos:narrower C2004A04997:318 ;
    skos:prefLabel "Chapter C379"@en-AU ;
    dcat:accessURL <https://www.legislation.gov.au/C2004A04997/2024-07-01/2024-07-01/text/1/epub/OEBPS/document_5/document_5.html#_Toc171753221> ;
    dcat:landingPage "https://www.legislation.gov.au/C2004A04997/2024-07-01/2024-07-01/text/1/epub/OEBPS/document_5/document_5.html#_Toc171753221"^^xsd:anyURI ;
    dcat:theme legcons:Chapter .

C2004A04997:38 a legcons:Item,
        C2004A04997:Item,
        owl:Class,
        dcat:Resource ;
    rdfs:label "Item - I38 16  Calculation of duty"@en-AU ;
    dct:isPartOf C2004A04997:36 ;
    rdfs:comment "16  Calculation of duty - Abrievated Graph Key: I38"@en-AU ;
    rdfs:subClassOf C2004A04997: ;
    skos:definition "16  Calculation of duty"@en-AU ;
    skos:narrower C2004A04997:36 ;
    skos:prefLabel "Item I38"@en-AU ;
    dcat:accessURL <https://www.legislation.gov.au/C2004A04997/2024-07-01/2024-07-01/text/1/epub/OEBPS/document_1/document_1.html#_Toc172806538> ;
    dcat:landingPage "https://www.legislation.gov.au/C2004A04997/2024-07-01/2024-07-01/text/1/epub/OEBPS/document_1/document_1.html#_Toc172806538"^^xsd:anyURI ;
    dcat:theme legcons:Item .

C2004A04997:380 a legcons:Item,
        C2004A04997:Item,
        owl:Class,
        dcat:Resource ;
    rdfs:label "Item - I380 Notes"@en-AU ;
    dct:isPartOf C2004A04997:318 ;
    rdfs:comment "Notes - Abrievated Graph Key: I380"@en-AU ;
    rdfs:subClassOf C2004A04997: ;
    skos:definition "Notes"@en-AU ;
    skos:narrower C2004A04997:318 ;
    skos:prefLabel "Item I380"@en-AU ;
    dcat:accessURL <https://www.legislation.gov.au/C2004A04997/2024-07-01/2024-07-01/text/1/epub/OEBPS/document_5/document_5.html#_Toc171753222> ;
    dcat:landingPage "https://www.legislation.gov.au/C2004A04997/2024-07-01/2024-07-01/text/1/epub/OEBPS/document_5/document_5.html#_Toc171753222"^^xsd:anyURI ;
    dcat:theme legcons:Item .

C2004A04997:381 a legcons:Item,
        C2004A04997:Item,
        owl:Class,
        dcat:Resource ;
    rdfs:label "Item - I381 Subheading Note"@en-AU ;
    dct:isPartOf C2004A04997:318 ;
    rdfs:comment "Subheading Note - Abrievated Graph Key: I381"@en-AU ;
    rdfs:subClassOf C2004A04997: ;
    skos:definition "Subheading Note"@en-AU ;
    skos:narrower C2004A04997:318 ;
    skos:prefLabel "Item I381"@en-AU ;
    dcat:accessURL <https://www.legislation.gov.au/C2004A04997/2024-07-01/2024-07-01/text/1/epub/OEBPS/document_5/document_5.html#_Toc171753223> ;
    dcat:landingPage "https://www.legislation.gov.au/C2004A04997/2024-07-01/2024-07-01/text/1/epub/OEBPS/document_5/document_5.html#_Toc171753223"^^xsd:anyURI ;
    dcat:theme legcons:Item .

C2004A04997:382 a legcons:Chapter,
        C2004A04997:Chapter,
        owl:Class,
        dcat:Resource ;
    rdfs:label "Chapter - C382 Chapter 96 Miscellaneous manufactured articles"@en-AU ;
    dct:isPartOf C2004A04997:318 ;
    rdfs:comment "Chapter 96 Miscellaneous manufactured articles - Abrievated Graph Key: C382"@en-AU ;
    rdfs:subClassOf C2004A04997: ;
    skos:definition "Chapter 96 Miscellaneous manufactured articles"@en-AU ;
    skos:narrower C2004A04997:318 ;
    skos:prefLabel "Chapter C382"@en-AU ;
    dcat:accessURL <https://www.legislation.gov.au/C2004A04997/2024-07-01/2024-07-01/text/1/epub/OEBPS/document_5/document_5.html#_Toc171753224> ;
    dcat:landingPage "https://www.legislation.gov.au/C2004A04997/2024-07-01/2024-07-01/text/1/epub/OEBPS/document_5/document_5.html#_Toc171753224"^^xsd:anyURI ;
    dcat:theme legcons:Chapter .

C2004A04997:383 a legcons:Item,
        C2004A04997:Item,
        owl:Class,
        dcat:Resource ;
    rdfs:label "Item - I383 Notes"@en-AU ;
    dct:isPartOf C2004A04997:318 ;
    rdfs:comment "Notes - Abrievated Graph Key: I383"@en-AU ;
    rdfs:subClassOf C2004A04997: ;
    skos:definition "Notes"@en-AU ;
    skos:narrower C2004A04997:318 ;
    skos:prefLabel "Item I383"@en-AU ;
    dcat:accessURL <https://www.legislation.gov.au/C2004A04997/2024-07-01/2024-07-01/text/1/epub/OEBPS/document_5/document_5.html#_Toc171753225> ;
    dcat:landingPage "https://www.legislation.gov.au/C2004A04997/2024-07-01/2024-07-01/text/1/epub/OEBPS/document_5/document_5.html#_Toc171753225"^^xsd:anyURI ;
    dcat:theme legcons:Item .

C2004A04997:384 a legcons:Section,
        C2004A04997:Section,
        owl:Class,
        dcat:Resource ;
    rdfs:label "Section - S384 Section XXIWorks of art collectors pieces and antiques"@en-AU ;
    dct:isPartOf C2004A04997:318 ;
    rdfs:comment "Section XXIWorks of art collectors pieces and antiques - Abrievated Graph Key: S384"@en-AU ;
    rdfs:subClassOf C2004A04997: ;
    skos:definition "Section XXIWorks of art collectors pieces and antiques"@en-AU ;
    skos:narrower C2004A04997:318 ;
    skos:prefLabel "Section S384"@en-AU ;
    dcat:accessURL <https://www.legislation.gov.au/C2004A04997/2024-07-01/2024-07-01/text/1/epub/OEBPS/document_5/document_5.html#_Toc171753226> ;
    dcat:landingPage "https://www.legislation.gov.au/C2004A04997/2024-07-01/2024-07-01/text/1/epub/OEBPS/document_5/document_5.html#_Toc171753226"^^xsd:anyURI ;
    dcat:theme legcons:Section .

C2004A04997:385 a legcons:Chapter,
        C2004A04997:Chapter,
        owl:Class,
        dcat:Resource ;
    rdfs:label "Chapter - C385 Chapter 97 Works of art collectors pieces and antiques"@en-AU ;
    dct:isPartOf C2004A04997:318 ;
    rdfs:comment "Chapter 97 Works of art collectors pieces and antiques - Abrievated Graph Key: C385"@en-AU ;
    rdfs:subClassOf C2004A04997: ;
    skos:definition "Chapter 97 Works of art collectors pieces and antiques"@en-AU ;
    skos:narrower C2004A04997:318 ;
    skos:prefLabel "Chapter C385"@en-AU ;
    dcat:accessURL <https://www.legislation.gov.au/C2004A04997/2024-07-01/2024-07-01/text/1/epub/OEBPS/document_5/document_5.html#_Toc171753227> ;
    dcat:landingPage "https://www.legislation.gov.au/C2004A04997/2024-07-01/2024-07-01/text/1/epub/OEBPS/document_5/document_5.html#_Toc171753227"^^xsd:anyURI ;
    dcat:theme legcons:Chapter .

C2004A04997:386 a legcons:Item,
        C2004A04997:Item,
        owl:Class,
        dcat:Resource ;
    rdfs:label "Item - I386 Notes"@en-AU ;
    dct:isPartOf C2004A04997:318 ;
    rdfs:comment "Notes - Abrievated Graph Key: I386"@en-AU ;
    rdfs:subClassOf C2004A04997: ;
    skos:definition "Notes"@en-AU ;
    skos:narrower C2004A04997:318 ;
    skos:prefLabel "Item I386"@en-AU ;
    dcat:accessURL <https://www.legislation.gov.au/C2004A04997/2024-07-01/2024-07-01/text/1/epub/OEBPS/document_5/document_5.html#_Toc171753228> ;
    dcat:landingPage "https://www.legislation.gov.au/C2004A04997/2024-07-01/2024-07-01/text/1/epub/OEBPS/document_5/document_5.html#_Toc171753228"^^xsd:anyURI ;
    dcat:theme legcons:Item .

C2004A04997:387 a legcons:Item,
        C2004A04997:Item,
        owl:Class,
        dcat:Resource ;
    rdfs:label "Item - I387 Additional Notes"@en-AU ;
    dct:isPartOf C2004A04997:318 ;
    rdfs:comment "Additional Notes - Abrievated Graph Key: I387"@en-AU ;
    rdfs:subClassOf C2004A04997: ;
    skos:definition "Additional Notes"@en-AU ;
    skos:narrower C2004A04997:318 ;
    skos:prefLabel "Item I387"@en-AU ;
    dcat:accessURL <https://www.legislation.gov.au/C2004A04997/2024-07-01/2024-07-01/text/1/epub/OEBPS/document_5/document_5.html#_Toc171753229> ;
    dcat:landingPage "https://www.legislation.gov.au/C2004A04997/2024-07-01/2024-07-01/text/1/epub/OEBPS/document_5/document_5.html#_Toc171753229"^^xsd:anyURI ;
    dcat:theme legcons:Item .

C2004A04997:389 a legcons:Schedule,
        C2004A04997:Schedule,
        owl:Class,
        dcat:Resource ;
    rdfs:label "Schedule - S389 Schedule 4 Concessional rates of duty"@en-AU ;
    dct:isPartOf C2004A04997:388 ;
    rdfs:comment "Schedule 4 Concessional rates of duty - Abrievated Graph Key: S389"@en-AU ;
    rdfs:subClassOf C2004A04997: ;
    skos:definition "Schedule 4 Concessional rates of duty"@en-AU ;
    skos:narrower C2004A04997:388 ;
    skos:prefLabel "Schedule S389"@en-AU ;
    dcat:accessURL <https://www.legislation.gov.au/C2004A04997/2024-07-01/2024-07-01/text/1/epub/OEBPS/document_6/document_6.html#_Toc171754999> ;
    dcat:landingPage "https://www.legislation.gov.au/C2004A04997/2024-07-01/2024-07-01/text/1/epub/OEBPS/document_6/document_6.html#_Toc171754999"^^xsd:anyURI ;
    dcat:theme legcons:Schedule .

C2004A04997:39 a legcons:Item,
        C2004A04997:Item,
        owl:Class,
        dcat:Resource ;
    rdfs:label "Item - I39 16 A  Suspension of preferential tariff for UK originating goodssafeguard goods"@en-AU ;
    dct:isPartOf C2004A04997:36 ;
    rdfs:comment "16 A  Suspension of preferential tariff for UK originating goodssafeguard goods - Abrievated Graph Key: I39"@en-AU ;
    rdfs:subClassOf C2004A04997: ;
    skos:definition "16 A  Suspension of preferential tariff for UK originating goodssafeguard goods"@en-AU ;
    skos:narrower C2004A04997:36 ;
    skos:prefLabel "Item I39"@en-AU ;
    dcat:accessURL <https://www.legislation.gov.au/C2004A04997/2024-07-01/2024-07-01/text/1/epub/OEBPS/document_1/document_1.html#_Toc172806539> ;
    dcat:landingPage "https://www.legislation.gov.au/C2004A04997/2024-07-01/2024-07-01/text/1/epub/OEBPS/document_1/document_1.html#_Toc172806539"^^xsd:anyURI ;
    dcat:theme legcons:Item .

C2004A04997:390 a legcons:Schedule,
        C2004A04997:Schedule,
        owl:Class,
        dcat:Resource ;
    rdfs:label "Schedule - S390 Schedule 4 ASingaporean originating goods"@en-AU ;
    dct:isPartOf C2004A04997:388 ;
    rdfs:comment "Schedule 4 ASingaporean originating goods - Abrievated Graph Key: S390"@en-AU ;
    rdfs:subClassOf C2004A04997: ;
    skos:definition "Schedule 4 ASingaporean originating goods"@en-AU ;
    skos:narrower C2004A04997:388 ;
    skos:prefLabel "Schedule S390"@en-AU ;
    dcat:accessURL <https://www.legislation.gov.au/C2004A04997/2024-07-01/2024-07-01/text/1/epub/OEBPS/document_6/document_6.html#_Toc171755000> ;
    dcat:landingPage "https://www.legislation.gov.au/C2004A04997/2024-07-01/2024-07-01/text/1/epub/OEBPS/document_6/document_6.html#_Toc171755000"^^xsd:anyURI ;
    dcat:theme legcons:Schedule .

C2004A04997:391 a legcons:Schedule,
        C2004A04997:Schedule,
        owl:Class,
        dcat:Resource ;
    rdfs:label "Schedule - S391 Schedule 5 US originating goods"@en-AU ;
    dct:isPartOf C2004A04997:388 ;
    rdfs:comment "Schedule 5 US originating goods - Abrievated Graph Key: S391"@en-AU ;
    rdfs:subClassOf C2004A04997: ;
    skos:definition "Schedule 5 US originating goods"@en-AU ;
    skos:narrower C2004A04997:388 ;
    skos:prefLabel "Schedule S391"@en-AU ;
    dcat:accessURL <https://www.legislation.gov.au/C2004A04997/2024-07-01/2024-07-01/text/1/epub/OEBPS/document_6/document_6.html#_Toc171755001> ;
    dcat:landingPage "https://www.legislation.gov.au/C2004A04997/2024-07-01/2024-07-01/text/1/epub/OEBPS/document_6/document_6.html#_Toc171755001"^^xsd:anyURI ;
    dcat:theme legcons:Schedule .

C2004A04997:392 a legcons:Schedule,
        C2004A04997:Schedule,
        owl:Class,
        dcat:Resource ;
    rdfs:label "Schedule - S392 Schedule 6 Thai originating goods"@en-AU ;
    dct:isPartOf C2004A04997:388 ;
    rdfs:comment "Schedule 6 Thai originating goods - Abrievated Graph Key: S392"@en-AU ;
    rdfs:subClassOf C2004A04997: ;
    skos:definition "Schedule 6 Thai originating goods"@en-AU ;
    skos:narrower C2004A04997:388 ;
    skos:prefLabel "Schedule S392"@en-AU ;
    dcat:accessURL <https://www.legislation.gov.au/C2004A04997/2024-07-01/2024-07-01/text/1/epub/OEBPS/document_6/document_6.html#_Toc171755002> ;
    dcat:landingPage "https://www.legislation.gov.au/C2004A04997/2024-07-01/2024-07-01/text/1/epub/OEBPS/document_6/document_6.html#_Toc171755002"^^xsd:anyURI ;
    dcat:theme legcons:Schedule .

C2004A04997:393 a legcons:Schedule,
        C2004A04997:Schedule,
        owl:Class,
        dcat:Resource ;
    rdfs:label "Schedule - S393 Schedule 6 APeruvian originating goods"@en-AU ;
    dct:isPartOf C2004A04997:388 ;
    rdfs:comment "Schedule 6 APeruvian originating goods - Abrievated Graph Key: S393"@en-AU ;
    rdfs:subClassOf C2004A04997: ;
    skos:definition "Schedule 6 APeruvian originating goods"@en-AU ;
    skos:narrower C2004A04997:388 ;
    skos:prefLabel "Schedule S393"@en-AU ;
    dcat:accessURL <https://www.legislation.gov.au/C2004A04997/2024-07-01/2024-07-01/text/1/epub/OEBPS/document_6/document_6.html#_Toc171755003> ;
    dcat:landingPage "https://www.legislation.gov.au/C2004A04997/2024-07-01/2024-07-01/text/1/epub/OEBPS/document_6/document_6.html#_Toc171755003"^^xsd:anyURI ;
    dcat:theme legcons:Schedule .

C2004A04997:394 a legcons:Schedule,
        C2004A04997:Schedule,
        owl:Class,
        dcat:Resource ;
    rdfs:label "Schedule - S394 Schedule 7 Chilean originating goods"@en-AU ;
    dct:isPartOf C2004A04997:388 ;
    rdfs:comment "Schedule 7 Chilean originating goods - Abrievated Graph Key: S394"@en-AU ;
    rdfs:subClassOf C2004A04997: ;
    skos:definition "Schedule 7 Chilean originating goods"@en-AU ;
    skos:narrower C2004A04997:388 ;
    skos:prefLabel "Schedule S394"@en-AU ;
    dcat:accessURL <https://www.legislation.gov.au/C2004A04997/2024-07-01/2024-07-01/text/1/epub/OEBPS/document_6/document_6.html#_Toc171755004> ;
    dcat:landingPage "https://www.legislation.gov.au/C2004A04997/2024-07-01/2024-07-01/text/1/epub/OEBPS/document_6/document_6.html#_Toc171755004"^^xsd:anyURI ;
    dcat:theme legcons:Schedule .

C2004A04997:395 a legcons:Schedule,
        C2004A04997:Schedule,
        owl:Class,
        dcat:Resource ;
    rdfs:label "Schedule - S395 Schedule 8 ASEAN Australia New Zealand AANZ originating goods"@en-AU ;
    dct:isPartOf C2004A04997:388 ;
    rdfs:comment "Schedule 8 ASEAN Australia New Zealand AANZ originating goods - Abrievated Graph Key: S395"@en-AU ;
    rdfs:subClassOf C2004A04997: ;
    skos:definition "Schedule 8 ASEAN Australia New Zealand AANZ originating goods"@en-AU ;
    skos:narrower C2004A04997:388 ;
    skos:prefLabel "Schedule S395"@en-AU ;
    dcat:accessURL <https://www.legislation.gov.au/C2004A04997/2024-07-01/2024-07-01/text/1/epub/OEBPS/document_6/document_6.html#_Toc171755005> ;
    dcat:landingPage "https://www.legislation.gov.au/C2004A04997/2024-07-01/2024-07-01/text/1/epub/OEBPS/document_6/document_6.html#_Toc171755005"^^xsd:anyURI ;
    dcat:theme legcons:Schedule .

C2004A04997:396 a legcons:Schedule,
        C2004A04997:Schedule,
        owl:Class,
        dcat:Resource ;
    rdfs:label "Schedule - S396 Schedule 8 APacific Islands originating goods"@en-AU ;
    dct:isPartOf C2004A04997:388 ;
    rdfs:comment "Schedule 8 APacific Islands originating goods - Abrievated Graph Key: S396"@en-AU ;
    rdfs:subClassOf C2004A04997: ;
    skos:definition "Schedule 8 APacific Islands originating goods"@en-AU ;
    skos:narrower C2004A04997:388 ;
    skos:prefLabel "Schedule S396"@en-AU ;
    dcat:accessURL <https://www.legislation.gov.au/C2004A04997/2024-07-01/2024-07-01/text/1/epub/OEBPS/document_6/document_6.html#_Toc171755006> ;
    dcat:landingPage "https://www.legislation.gov.au/C2004A04997/2024-07-01/2024-07-01/text/1/epub/OEBPS/document_6/document_6.html#_Toc171755006"^^xsd:anyURI ;
    dcat:theme legcons:Schedule .

C2004A04997:397 a legcons:Schedule,
        C2004A04997:Schedule,
        owl:Class,
        dcat:Resource ;
    rdfs:label "Schedule - S397 Schedule 8 BTrans Pacific Partnership originating goods"@en-AU ;
    dct:isPartOf C2004A04997:388 ;
    rdfs:comment "Schedule 8 BTrans Pacific Partnership originating goods - Abrievated Graph Key: S397"@en-AU ;
    rdfs:subClassOf C2004A04997: ;
    skos:definition "Schedule 8 BTrans Pacific Partnership originating goods"@en-AU ;
    skos:narrower C2004A04997:388 ;
    skos:prefLabel "Schedule S397"@en-AU ;
    dcat:accessURL <https://www.legislation.gov.au/C2004A04997/2024-07-01/2024-07-01/text/1/epub/OEBPS/document_6/document_6.html#_Toc171755007> ;
    dcat:landingPage "https://www.legislation.gov.au/C2004A04997/2024-07-01/2024-07-01/text/1/epub/OEBPS/document_6/document_6.html#_Toc171755007"^^xsd:anyURI ;
    dcat:theme legcons:Schedule .

C2004A04997:398 a legcons:Schedule,
        C2004A04997:Schedule,
        owl:Class,
        dcat:Resource ;
    rdfs:label "Schedule - S398 Schedule 9 Malaysian originating goods"@en-AU ;
    dct:isPartOf C2004A04997:388 ;
    rdfs:comment "Schedule 9 Malaysian originating goods - Abrievated Graph Key: S398"@en-AU ;
    rdfs:subClassOf C2004A04997: ;
    skos:definition "Schedule 9 Malaysian originating goods"@en-AU ;
    skos:narrower C2004A04997:388 ;
    skos:prefLabel "Schedule S398"@en-AU ;
    dcat:accessURL <https://www.legislation.gov.au/C2004A04997/2024-07-01/2024-07-01/text/1/epub/OEBPS/document_6/document_6.html#_Toc171755008> ;
    dcat:landingPage "https://www.legislation.gov.au/C2004A04997/2024-07-01/2024-07-01/text/1/epub/OEBPS/document_6/document_6.html#_Toc171755008"^^xsd:anyURI ;
    dcat:theme legcons:Schedule .

C2004A04997:399 a legcons:Schedule,
        C2004A04997:Schedule,
        owl:Class,
        dcat:Resource ;
    rdfs:label "Schedule - S399 Schedule 9 AIndonesian originating goods"@en-AU ;
    dct:isPartOf C2004A04997:388 ;
    rdfs:comment "Schedule 9 AIndonesian originating goods - Abrievated Graph Key: S399"@en-AU ;
    rdfs:subClassOf C2004A04997: ;
    skos:definition "Schedule 9 AIndonesian originating goods"@en-AU ;
    skos:narrower C2004A04997:388 ;
    skos:prefLabel "Schedule S399"@en-AU ;
    dcat:accessURL <https://www.legislation.gov.au/C2004A04997/2024-07-01/2024-07-01/text/1/epub/OEBPS/document_6/document_6.html#_Toc171755009> ;
    dcat:landingPage "https://www.legislation.gov.au/C2004A04997/2024-07-01/2024-07-01/text/1/epub/OEBPS/document_6/document_6.html#_Toc171755009"^^xsd:anyURI ;
    dcat:theme legcons:Schedule .

C2004A04997:4 a legcons:Item,
        C2004A04997:Item,
        owl:Class,
        dcat:Resource ;
    rdfs:label "Item - I4 2  Commencement"@en-AU ;
    dct:isPartOf C2004A04997:2 ;
    rdfs:comment "2  Commencement - Abrievated Graph Key: I4"@en-AU ;
    rdfs:subClassOf C2004A04997: ;
    skos:definition "2  Commencement"@en-AU ;
    skos:narrower C2004A04997:2 ;
    skos:prefLabel "Item I4"@en-AU ;
    dcat:accessURL <https://www.legislation.gov.au/C2004A04997/2024-07-01/2024-07-01/text/1/epub/OEBPS/document_1/document_1.html#_Toc172806504> ;
    dcat:landingPage "https://www.legislation.gov.au/C2004A04997/2024-07-01/2024-07-01/text/1/epub/OEBPS/document_1/document_1.html#_Toc172806504"^^xsd:anyURI ;
    dcat:theme legcons:Item .

C2004A04997:40 a legcons:Item,
        C2004A04997:Item,
        owl:Class,
        dcat:Resource ;
    rdfs:label "Item - I40 17  Rates for goods with constituents etc"@en-AU ;
    dct:isPartOf C2004A04997:36 ;
    rdfs:comment "17  Rates for goods with constituents etc - Abrievated Graph Key: I40"@en-AU ;
    rdfs:subClassOf C2004A04997: ;
    skos:definition "17  Rates for goods with constituents etc"@en-AU ;
    skos:narrower C2004A04997:36 ;
    skos:prefLabel "Item I40"@en-AU ;
    dcat:accessURL <https://www.legislation.gov.au/C2004A04997/2024-07-01/2024-07-01/text/1/epub/OEBPS/document_1/document_1.html#_Toc172806540> ;
    dcat:landingPage "https://www.legislation.gov.au/C2004A04997/2024-07-01/2024-07-01/text/1/epub/OEBPS/document_1/document_1.html#_Toc172806540"^^xsd:anyURI ;
    dcat:theme legcons:Item .

C2004A04997:400 a legcons:Schedule,
        C2004A04997:Schedule,
        owl:Class,
        dcat:Resource ;
    rdfs:label "Schedule - S400 Schedule 10 Korean originating goods"@en-AU ;
    dct:isPartOf C2004A04997:388 ;
    rdfs:comment "Schedule 10 Korean originating goods - Abrievated Graph Key: S400"@en-AU ;
    rdfs:subClassOf C2004A04997: ;
    skos:definition "Schedule 10 Korean originating goods"@en-AU ;
    skos:narrower C2004A04997:388 ;
    skos:prefLabel "Schedule S400"@en-AU ;
    dcat:accessURL <https://www.legislation.gov.au/C2004A04997/2024-07-01/2024-07-01/text/1/epub/OEBPS/document_6/document_6.html#_Toc171755010> ;
    dcat:landingPage "https://www.legislation.gov.au/C2004A04997/2024-07-01/2024-07-01/text/1/epub/OEBPS/document_6/document_6.html#_Toc171755010"^^xsd:anyURI ;
    dcat:theme legcons:Schedule .

C2004A04997:401 a legcons:Schedule,
        C2004A04997:Schedule,
        owl:Class,
        dcat:Resource ;
    rdfs:label "Schedule - S401 Schedule 10 AIndian originating goods"@en-AU ;
    dct:isPartOf C2004A04997:388 ;
    rdfs:comment "Schedule 10 AIndian originating goods - Abrievated Graph Key: S401"@en-AU ;
    rdfs:subClassOf C2004A04997: ;
    skos:definition "Schedule 10 AIndian originating goods"@en-AU ;
    skos:narrower C2004A04997:388 ;
    skos:prefLabel "Schedule S401"@en-AU ;
    dcat:accessURL <https://www.legislation.gov.au/C2004A04997/2024-07-01/2024-07-01/text/1/epub/OEBPS/document_6/document_6.html#_Toc171755011> ;
    dcat:landingPage "https://www.legislation.gov.au/C2004A04997/2024-07-01/2024-07-01/text/1/epub/OEBPS/document_6/document_6.html#_Toc171755011"^^xsd:anyURI ;
    dcat:theme legcons:Schedule .

C2004A04997:402 a legcons:Schedule,
        C2004A04997:Schedule,
        owl:Class,
        dcat:Resource ;
    rdfs:label "Schedule - S402 Schedule 11 Japanese originating goods"@en-AU ;
    dct:isPartOf C2004A04997:388 ;
    rdfs:comment "Schedule 11 Japanese originating goods - Abrievated Graph Key: S402"@en-AU ;
    rdfs:subClassOf C2004A04997: ;
    skos:definition "Schedule 11 Japanese originating goods"@en-AU ;
    skos:narrower C2004A04997:388 ;
    skos:prefLabel "Schedule S402"@en-AU ;
    dcat:accessURL <https://www.legislation.gov.au/C2004A04997/2024-07-01/2024-07-01/text/1/epub/OEBPS/document_6/document_6.html#_Toc171755012> ;
    dcat:landingPage "https://www.legislation.gov.au/C2004A04997/2024-07-01/2024-07-01/text/1/epub/OEBPS/document_6/document_6.html#_Toc171755012"^^xsd:anyURI ;
    dcat:theme legcons:Schedule .

C2004A04997:403 a legcons:Schedule,
        C2004A04997:Schedule,
        owl:Class,
        dcat:Resource ;
    rdfs:label "Schedule - S403 Schedule 12 Chinese originating goods"@en-AU ;
    dct:isPartOf C2004A04997:388 ;
    rdfs:comment "Schedule 12 Chinese originating goods - Abrievated Graph Key: S403"@en-AU ;
    rdfs:subClassOf C2004A04997: ;
    skos:definition "Schedule 12 Chinese originating goods"@en-AU ;
    skos:narrower C2004A04997:388 ;
    skos:prefLabel "Schedule S403"@en-AU ;
    dcat:accessURL <https://www.legislation.gov.au/C2004A04997/2024-07-01/2024-07-01/text/1/epub/OEBPS/document_6/document_6.html#_Toc171755013> ;
    dcat:landingPage "https://www.legislation.gov.au/C2004A04997/2024-07-01/2024-07-01/text/1/epub/OEBPS/document_6/document_6.html#_Toc171755013"^^xsd:anyURI ;
    dcat:theme legcons:Schedule .

C2004A04997:404 a legcons:Schedule,
        C2004A04997:Schedule,
        owl:Class,
        dcat:Resource ;
    rdfs:label "Schedule - S404 Schedule 13 Hong Kong originating goods"@en-AU ;
    dct:isPartOf C2004A04997:388 ;
    rdfs:comment "Schedule 13 Hong Kong originating goods - Abrievated Graph Key: S404"@en-AU ;
    rdfs:subClassOf C2004A04997: ;
    skos:definition "Schedule 13 Hong Kong originating goods"@en-AU ;
    skos:narrower C2004A04997:388 ;
    skos:prefLabel "Schedule S404"@en-AU ;
    dcat:accessURL <https://www.legislation.gov.au/C2004A04997/2024-07-01/2024-07-01/text/1/epub/OEBPS/document_6/document_6.html#_Toc171755014> ;
    dcat:landingPage "https://www.legislation.gov.au/C2004A04997/2024-07-01/2024-07-01/text/1/epub/OEBPS/document_6/document_6.html#_Toc171755014"^^xsd:anyURI ;
    dcat:theme legcons:Schedule .

C2004A04997:405 a legcons:Schedule,
        C2004A04997:Schedule,
        owl:Class,
        dcat:Resource ;
    rdfs:label "Schedule - S405 Schedule 14 Regional Comprehensive Economic Partnership RCEP originating goods"@en-AU ;
    dct:isPartOf C2004A04997:388 ;
    rdfs:comment "Schedule 14 Regional Comprehensive Economic Partnership RCEP originating goods - Abrievated Graph Key: S405"@en-AU ;
    rdfs:subClassOf C2004A04997: ;
    skos:definition "Schedule 14 Regional Comprehensive Economic Partnership RCEP originating goods"@en-AU ;
    skos:narrower C2004A04997:388 ;
    skos:prefLabel "Schedule S405"@en-AU ;
    dcat:accessURL <https://www.legislation.gov.au/C2004A04997/2024-07-01/2024-07-01/text/1/epub/OEBPS/document_6/document_6.html#_Toc171755015> ;
    dcat:landingPage "https://www.legislation.gov.au/C2004A04997/2024-07-01/2024-07-01/text/1/epub/OEBPS/document_6/document_6.html#_Toc171755015"^^xsd:anyURI ;
    dcat:theme legcons:Schedule .

C2004A04997:406 a legcons:Schedule,
        C2004A04997:Schedule,
        owl:Class,
        dcat:Resource ;
    rdfs:label "Schedule - S406 Schedule 15 UK originating goods"@en-AU ;
    dct:isPartOf C2004A04997:388 ;
    rdfs:comment "Schedule 15 UK originating goods - Abrievated Graph Key: S406"@en-AU ;
    rdfs:subClassOf C2004A04997: ;
    skos:definition "Schedule 15 UK originating goods"@en-AU ;
    skos:narrower C2004A04997:388 ;
    skos:prefLabel "Schedule S406"@en-AU ;
    dcat:accessURL <https://www.legislation.gov.au/C2004A04997/2024-07-01/2024-07-01/text/1/epub/OEBPS/document_6/document_6.html#_Toc171755016> ;
    dcat:landingPage "https://www.legislation.gov.au/C2004A04997/2024-07-01/2024-07-01/text/1/epub/OEBPS/document_6/document_6.html#_Toc171755016"^^xsd:anyURI ;
    dcat:theme legcons:Schedule .

C2004A04997:407 a legcons:Volume,
        C2004A04997:Volume,
        owl:Class,
        dcat:Resource ;
    rdfs:label "Volume - V407 Volume 7"@en-AU ;
    dct:hasPart C2004A04997:408 ;
    rdfs:comment "Volume 7 - Abrievated Graph Key: V407"@en-AU ;
    rdfs:subClassOf C2004A04997: ;
    skos:broader C2004A04997:408 ;
    skos:definition "Volume 7"@en-AU ;
    skos:prefLabel "Volume V407"@en-AU ;
    dcat:accessURL <https://www.legislation.gov.au/C2004A04997/2024-07-01/2024-07-01/text/1/epub/OEBPS/document_7/document_7.html> ;
    dcat:landingPage "https://www.legislation.gov.au/C2004A04997/2024-07-01/2024-07-01/text/1/epub/OEBPS/document_7/document_7.html"^^xsd:anyURI ;
    dcat:theme legcons:Volume .

C2004A04997:409 a legcons:Item,
        C2004A04997:Item,
        owl:Class,
        dcat:Resource ;
    rdfs:label "Item - I409 Endnote 1 About the endnotes"@en-AU ;
    dct:isPartOf C2004A04997:408 ;
    rdfs:comment "Endnote 1 About the endnotes - Abrievated Graph Key: I409"@en-AU ;
    rdfs:subClassOf C2004A04997: ;
    skos:definition "Endnote 1 About the endnotes"@en-AU ;
    skos:narrower C2004A04997:408 ;
    skos:prefLabel "Item I409"@en-AU ;
    dcat:accessURL <https://www.legislation.gov.au/C2004A04997/2024-07-01/2024-07-01/text/1/epub/OEBPS/document_7/document_7.html#_Toc171755739> ;
    dcat:landingPage "https://www.legislation.gov.au/C2004A04997/2024-07-01/2024-07-01/text/1/epub/OEBPS/document_7/document_7.html#_Toc171755739"^^xsd:anyURI ;
    dcat:theme legcons:Item .

C2004A04997:41 a legcons:Item,
        C2004A04997:Item,
        owl:Class,
        dcat:Resource ;
    rdfs:label "Item - I41 18  Calculation of concessional duty"@en-AU ;
    dct:isPartOf C2004A04997:36 ;
    rdfs:comment "18  Calculation of concessional duty - Abrievated Graph Key: I41"@en-AU ;
    rdfs:subClassOf C2004A04997: ;
    skos:definition "18  Calculation of concessional duty"@en-AU ;
    skos:narrower C2004A04997:36 ;
    skos:prefLabel "Item I41"@en-AU ;
    dcat:accessURL <https://www.legislation.gov.au/C2004A04997/2024-07-01/2024-07-01/text/1/epub/OEBPS/document_1/document_1.html#_Toc172806541> ;
    dcat:landingPage "https://www.legislation.gov.au/C2004A04997/2024-07-01/2024-07-01/text/1/epub/OEBPS/document_1/document_1.html#_Toc172806541"^^xsd:anyURI ;
    dcat:theme legcons:Item .

C2004A04997:410 a legcons:Item,
        C2004A04997:Item,
        owl:Class,
        dcat:Resource ;
    rdfs:label "Item - I410 Endnote 2 Abbreviation key"@en-AU ;
    dct:isPartOf C2004A04997:408 ;
    rdfs:comment "Endnote 2 Abbreviation key - Abrievated Graph Key: I410"@en-AU ;
    rdfs:subClassOf C2004A04997: ;
    skos:definition "Endnote 2 Abbreviation key"@en-AU ;
    skos:narrower C2004A04997:408 ;
    skos:prefLabel "Item I410"@en-AU ;
    dcat:accessURL <https://www.legislation.gov.au/C2004A04997/2024-07-01/2024-07-01/text/1/epub/OEBPS/document_7/document_7.html#_Toc171755740> ;
    dcat:landingPage "https://www.legislation.gov.au/C2004A04997/2024-07-01/2024-07-01/text/1/epub/OEBPS/document_7/document_7.html#_Toc171755740"^^xsd:anyURI ;
    dcat:theme legcons:Item .

C2004A04997:411 a legcons:Item,
        C2004A04997:Item,
        owl:Class,
        dcat:Resource ;
    rdfs:label "Item - I411 Endnote 3 Legislation history"@en-AU ;
    dct:isPartOf C2004A04997:408 ;
    rdfs:comment "Endnote 3 Legislation history - Abrievated Graph Key: I411"@en-AU ;
    rdfs:subClassOf C2004A04997: ;
    skos:definition "Endnote 3 Legislation history"@en-AU ;
    skos:narrower C2004A04997:408 ;
    skos:prefLabel "Item I411"@en-AU ;
    dcat:accessURL <https://www.legislation.gov.au/C2004A04997/2024-07-01/2024-07-01/text/1/epub/OEBPS/document_7/document_7.html#_Toc171755741> ;
    dcat:landingPage "https://www.legislation.gov.au/C2004A04997/2024-07-01/2024-07-01/text/1/epub/OEBPS/document_7/document_7.html#_Toc171755741"^^xsd:anyURI ;
    dcat:theme legcons:Item .

C2004A04997:412 a legcons:Item,
        C2004A04997:Item,
        owl:Class,
        dcat:Resource ;
    rdfs:label "Item - I412 Endnote 4 Amendment history"@en-AU ;
    dct:isPartOf C2004A04997:408 ;
    rdfs:comment "Endnote 4 Amendment history - Abrievated Graph Key: I412"@en-AU ;
    rdfs:subClassOf C2004A04997: ;
    skos:definition "Endnote 4 Amendment history"@en-AU ;
    skos:narrower C2004A04997:408 ;
    skos:prefLabel "Item I412"@en-AU ;
    dcat:accessURL <https://www.legislation.gov.au/C2004A04997/2024-07-01/2024-07-01/text/1/epub/OEBPS/document_7/document_7.html#_Toc171755742> ;
    dcat:landingPage "https://www.legislation.gov.au/C2004A04997/2024-07-01/2024-07-01/text/1/epub/OEBPS/document_7/document_7.html#_Toc171755742"^^xsd:anyURI ;
    dcat:theme legcons:Item .

C2004A04997:42 a legcons:Item,
        C2004A04997:Item,
        owl:Class,
        dcat:Resource ;
    rdfs:label "Item - I42 18 A  Temporary increase in duties for goods from Russia or Belarus"@en-AU ;
    dct:isPartOf C2004A04997:36 ;
    rdfs:comment "18 A  Temporary increase in duties for goods from Russia or Belarus - Abrievated Graph Key: I42"@en-AU ;
    rdfs:subClassOf C2004A04997: ;
    skos:definition "18 A  Temporary increase in duties for goods from Russia or Belarus"@en-AU ;
    skos:narrower C2004A04997:36 ;
    skos:prefLabel "Item I42"@en-AU ;
    dcat:accessURL <https://www.legislation.gov.au/C2004A04997/2024-07-01/2024-07-01/text/1/epub/OEBPS/document_1/document_1.html#_Toc172806542> ;
    dcat:landingPage "https://www.legislation.gov.au/C2004A04997/2024-07-01/2024-07-01/text/1/epub/OEBPS/document_1/document_1.html#_Toc172806542"^^xsd:anyURI ;
    dcat:theme legcons:Item .

C2004A04997:43 a legcons:Item,
        C2004A04997:Item,
        owl:Class,
        dcat:Resource ;
    rdfs:label "Item - I43 18 B  Temporary decrease in duties for goods from Ukraine"@en-AU ;
    dct:isPartOf C2004A04997:36 ;
    rdfs:comment "18 B  Temporary decrease in duties for goods from Ukraine - Abrievated Graph Key: I43"@en-AU ;
    rdfs:subClassOf C2004A04997: ;
    skos:definition "18 B  Temporary decrease in duties for goods from Ukraine"@en-AU ;
    skos:narrower C2004A04997:36 ;
    skos:prefLabel "Item I43"@en-AU ;
    dcat:accessURL <https://www.legislation.gov.au/C2004A04997/2024-07-01/2024-07-01/text/1/epub/OEBPS/document_1/document_1.html#_Toc172806543> ;
    dcat:landingPage "https://www.legislation.gov.au/C2004A04997/2024-07-01/2024-07-01/text/1/epub/OEBPS/document_1/document_1.html#_Toc172806543"^^xsd:anyURI ;
    dcat:theme legcons:Item .

C2004A04997:44 a legcons:Item,
        C2004A04997:Item,
        owl:Class,
        dcat:Resource ;
    rdfs:label "Item - I44 19  Indexation of CPI indexed rates"@en-AU ;
    dct:isPartOf C2004A04997:36 ;
    rdfs:comment "19  Indexation of CPI indexed rates - Abrievated Graph Key: I44"@en-AU ;
    rdfs:subClassOf C2004A04997: ;
    skos:definition "19  Indexation of CPI indexed rates"@en-AU ;
    skos:narrower C2004A04997:36 ;
    skos:prefLabel "Item I44"@en-AU ;
    dcat:accessURL <https://www.legislation.gov.au/C2004A04997/2024-07-01/2024-07-01/text/1/epub/OEBPS/document_1/document_1.html#_Toc172806544> ;
    dcat:landingPage "https://www.legislation.gov.au/C2004A04997/2024-07-01/2024-07-01/text/1/epub/OEBPS/document_1/document_1.html#_Toc172806544"^^xsd:anyURI ;
    dcat:theme legcons:Item .

C2004A04997:45 a legcons:Item,
        C2004A04997:Item,
        owl:Class,
        dcat:Resource ;
    rdfs:label "Item - I45 19 AAA  Rounding of fuel duty rates"@en-AU ;
    dct:isPartOf C2004A04997:36 ;
    rdfs:comment "19 AAA  Rounding of fuel duty rates - Abrievated Graph Key: I45"@en-AU ;
    rdfs:subClassOf C2004A04997: ;
    skos:definition "19 AAA  Rounding of fuel duty rates"@en-AU ;
    skos:narrower C2004A04997:36 ;
    skos:prefLabel "Item I45"@en-AU ;
    dcat:accessURL <https://www.legislation.gov.au/C2004A04997/2024-07-01/2024-07-01/text/1/epub/OEBPS/document_1/document_1.html#_Toc172806545> ;
    dcat:landingPage "https://www.legislation.gov.au/C2004A04997/2024-07-01/2024-07-01/text/1/epub/OEBPS/document_1/document_1.html#_Toc172806545"^^xsd:anyURI ;
    dcat:theme legcons:Item .

C2004A04997:46 a legcons:Item,
        C2004A04997:Item,
        owl:Class,
        dcat:Resource ;
    rdfs:label "Item - I46 19 AAB  Change in fuel duty rates"@en-AU ;
    dct:isPartOf C2004A04997:36 ;
    rdfs:comment "19 AAB  Change in fuel duty rates - Abrievated Graph Key: I46"@en-AU ;
    rdfs:subClassOf C2004A04997: ;
    skos:definition "19 AAB  Change in fuel duty rates"@en-AU ;
    skos:narrower C2004A04997:36 ;
    skos:prefLabel "Item I46"@en-AU ;
    dcat:accessURL <https://www.legislation.gov.au/C2004A04997/2024-07-01/2024-07-01/text/1/epub/OEBPS/document_1/document_1.html#_Toc172806546> ;
    dcat:landingPage "https://www.legislation.gov.au/C2004A04997/2024-07-01/2024-07-01/text/1/epub/OEBPS/document_1/document_1.html#_Toc172806546"^^xsd:anyURI ;
    dcat:theme legcons:Item .

C2004A04997:47 a legcons:Item,
        C2004A04997:Item,
        owl:Class,
        dcat:Resource ;
    rdfs:label "Item - I47 19 AABA  Temporary reduction in indexed fuel duty rates"@en-AU ;
    dct:isPartOf C2004A04997:36 ;
    rdfs:comment "19 AABA  Temporary reduction in indexed fuel duty rates - Abrievated Graph Key: I47"@en-AU ;
    rdfs:subClassOf C2004A04997: ;
    skos:definition "19 AABA  Temporary reduction in indexed fuel duty rates"@en-AU ;
    skos:narrower C2004A04997:36 ;
    skos:prefLabel "Item I47"@en-AU ;
    dcat:accessURL <https://www.legislation.gov.au/C2004A04997/2024-07-01/2024-07-01/text/1/epub/OEBPS/document_1/document_1.html#_Toc172806547> ;
    dcat:landingPage "https://www.legislation.gov.au/C2004A04997/2024-07-01/2024-07-01/text/1/epub/OEBPS/document_1/document_1.html#_Toc172806547"^^xsd:anyURI ;
    dcat:theme legcons:Item .

C2004A04997:48 a legcons:Item,
        C2004A04997:Item,
        owl:Class,
        dcat:Resource ;
    rdfs:label "Item - I48 19 AABB  Temporary reduction in other duty rates"@en-AU ;
    dct:isPartOf C2004A04997:36 ;
    rdfs:comment "19 AABB  Temporary reduction in other duty rates - Abrievated Graph Key: I48"@en-AU ;
    rdfs:subClassOf C2004A04997: ;
    skos:definition "19 AABB  Temporary reduction in other duty rates"@en-AU ;
    skos:narrower C2004A04997:36 ;
    skos:prefLabel "Item I48"@en-AU ;
    dcat:accessURL <https://www.legislation.gov.au/C2004A04997/2024-07-01/2024-07-01/text/1/epub/OEBPS/document_1/document_1.html#_Toc172806548> ;
    dcat:landingPage "https://www.legislation.gov.au/C2004A04997/2024-07-01/2024-07-01/text/1/epub/OEBPS/document_1/document_1.html#_Toc172806548"^^xsd:anyURI ;
    dcat:theme legcons:Item .

C2004A04997:49 a legcons:Item,
        C2004A04997:Item,
        owl:Class,
        dcat:Resource ;
    rdfs:label "Item - I49 19 AAC  Fuel duty rates"@en-AU ;
    dct:isPartOf C2004A04997:36 ;
    rdfs:comment "19 AAC  Fuel duty rates - Abrievated Graph Key: I49"@en-AU ;
    rdfs:subClassOf C2004A04997: ;
    skos:definition "19 AAC  Fuel duty rates"@en-AU ;
    skos:narrower C2004A04997:36 ;
    skos:prefLabel "Item I49"@en-AU ;
    dcat:accessURL <https://www.legislation.gov.au/C2004A04997/2024-07-01/2024-07-01/text/1/epub/OEBPS/document_1/document_1.html#_Toc172806549> ;
    dcat:landingPage "https://www.legislation.gov.au/C2004A04997/2024-07-01/2024-07-01/text/1/epub/OEBPS/document_1/document_1.html#_Toc172806549"^^xsd:anyURI ;
    dcat:theme legcons:Item .

C2004A04997:5 a legcons:Item,
        C2004A04997:Item,
        owl:Class,
        dcat:Resource ;
    rdfs:label "Item - I5 3  Definitions"@en-AU ;
    dct:isPartOf C2004A04997:2 ;
    rdfs:comment "3  Definitions - Abrievated Graph Key: I5"@en-AU ;
    rdfs:subClassOf C2004A04997: ;
    skos:definition "3  Definitions"@en-AU ;
    skos:narrower C2004A04997:2 ;
    skos:prefLabel "Item I5"@en-AU ;
    dcat:accessURL <https://www.legislation.gov.au/C2004A04997/2024-07-01/2024-07-01/text/1/epub/OEBPS/document_1/document_1.html#_Toc172806505> ;
    dcat:landingPage "https://www.legislation.gov.au/C2004A04997/2024-07-01/2024-07-01/text/1/epub/OEBPS/document_1/document_1.html#_Toc172806505"^^xsd:anyURI ;
    dcat:theme legcons:Item .

C2004A04997:50 a legcons:Item,
        C2004A04997:Item,
        owl:Class,
        dcat:Resource ;
    rdfs:label "Item - I50 19 AA  Alcohol duty rates"@en-AU ;
    dct:isPartOf C2004A04997:36 ;
    rdfs:comment "19 AA  Alcohol duty rates - Abrievated Graph Key: I50"@en-AU ;
    rdfs:subClassOf C2004A04997: ;
    skos:definition "19 AA  Alcohol duty rates"@en-AU ;
    skos:narrower C2004A04997:36 ;
    skos:prefLabel "Item I50"@en-AU ;
    dcat:accessURL <https://www.legislation.gov.au/C2004A04997/2024-07-01/2024-07-01/text/1/epub/OEBPS/document_1/document_1.html#_Toc172806550> ;
    dcat:landingPage "https://www.legislation.gov.au/C2004A04997/2024-07-01/2024-07-01/text/1/epub/OEBPS/document_1/document_1.html#_Toc172806550"^^xsd:anyURI ;
    dcat:theme legcons:Item .

C2004A04997:51 a legcons:Item,
        C2004A04997:Item,
        owl:Class,
        dcat:Resource ;
    rdfs:label "Item - I51 19 AB  Indexation of tobacco duty rates"@en-AU ;
    dct:isPartOf C2004A04997:36 ;
    rdfs:comment "19 AB  Indexation of tobacco duty rates - Abrievated Graph Key: I51"@en-AU ;
    rdfs:subClassOf C2004A04997: ;
    skos:definition "19 AB  Indexation of tobacco duty rates"@en-AU ;
    skos:narrower C2004A04997:36 ;
    skos:prefLabel "Item I51"@en-AU ;
    dcat:accessURL <https://www.legislation.gov.au/C2004A04997/2024-07-01/2024-07-01/text/1/epub/OEBPS/document_1/document_1.html#_Toc172806551> ;
    dcat:landingPage "https://www.legislation.gov.au/C2004A04997/2024-07-01/2024-07-01/text/1/epub/OEBPS/document_1/document_1.html#_Toc172806551"^^xsd:anyURI ;
    dcat:theme legcons:Item .

C2004A04997:52 a legcons:Item,
        C2004A04997:Item,
        owl:Class,
        dcat:Resource ;
    rdfs:label "Item - I52 19 AC  List of tobacco duty rates to be indexed under section 19 AB"@en-AU ;
    dct:isPartOf C2004A04997:36 ;
    rdfs:comment "19 AC  List of tobacco duty rates to be indexed under section 19 AB - Abrievated Graph Key: I52"@en-AU ;
    rdfs:subClassOf C2004A04997: ;
    skos:definition "19 AC  List of tobacco duty rates to be indexed under section 19 AB"@en-AU ;
    skos:narrower C2004A04997:36 ;
    skos:prefLabel "Item I52"@en-AU ;
    dcat:accessURL <https://www.legislation.gov.au/C2004A04997/2024-07-01/2024-07-01/text/1/epub/OEBPS/document_1/document_1.html#_Toc172806552> ;
    dcat:landingPage "https://www.legislation.gov.au/C2004A04997/2024-07-01/2024-07-01/text/1/epub/OEBPS/document_1/document_1.html#_Toc172806552"^^xsd:anyURI ;
    dcat:theme legcons:Item .

C2004A04997:53 a legcons:Item,
        C2004A04997:Item,
        owl:Class,
        dcat:Resource ;
    rdfs:label "Item - I53 19 ACA  Other tobacco duty rates"@en-AU ;
    dct:isPartOf C2004A04997:36 ;
    rdfs:comment "19 ACA  Other tobacco duty rates - Abrievated Graph Key: I53"@en-AU ;
    rdfs:subClassOf C2004A04997: ;
    skos:definition "19 ACA  Other tobacco duty rates"@en-AU ;
    skos:narrower C2004A04997:36 ;
    skos:prefLabel "Item I53"@en-AU ;
    dcat:accessURL <https://www.legislation.gov.au/C2004A04997/2024-07-01/2024-07-01/text/1/epub/OEBPS/document_1/document_1.html#_Toc172806553> ;
    dcat:landingPage "https://www.legislation.gov.au/C2004A04997/2024-07-01/2024-07-01/text/1/epub/OEBPS/document_1/document_1.html#_Toc172806553"^^xsd:anyURI ;
    dcat:theme legcons:Item .

C2004A04997:54 a legcons:Item,
        C2004A04997:Item,
        owl:Class,
        dcat:Resource ;
    rdfs:label "Item - I54 19 AD  Change in duty rate of certain liquefied petroleum gases liquefied natural gases and compressed natural gases"@en-AU ;
    dct:isPartOf C2004A04997:36 ;
    rdfs:comment "19 AD  Change in duty rate of certain liquefied petroleum gases liquefied natural gases and compressed natural gases - Abrievated Graph Key: I54"@en-AU ;
    rdfs:subClassOf C2004A04997: ;
    skos:definition "19 AD  Change in duty rate of certain liquefied petroleum gases liquefied natural gases and compressed natural gases"@en-AU ;
    skos:narrower C2004A04997:36 ;
    skos:prefLabel "Item I54"@en-AU ;
    dcat:accessURL <https://www.legislation.gov.au/C2004A04997/2024-07-01/2024-07-01/text/1/epub/OEBPS/document_1/document_1.html#_Toc172806554> ;
    dcat:landingPage "https://www.legislation.gov.au/C2004A04997/2024-07-01/2024-07-01/text/1/epub/OEBPS/document_1/document_1.html#_Toc172806554"^^xsd:anyURI ;
    dcat:theme legcons:Item .

C2004A04997:55 a legcons:Item,
        C2004A04997:Item,
        owl:Class,
        dcat:Resource ;
    rdfs:label "Item - I55 20  Duty where goods consist of certain containers and certain contents"@en-AU ;
    dct:isPartOf C2004A04997:36 ;
    rdfs:comment "20  Duty where goods consist of certain containers and certain contents - Abrievated Graph Key: I55"@en-AU ;
    rdfs:subClassOf C2004A04997: ;
    skos:definition "20  Duty where goods consist of certain containers and certain contents"@en-AU ;
    skos:narrower C2004A04997:36 ;
    skos:prefLabel "Item I55"@en-AU ;
    dcat:accessURL <https://www.legislation.gov.au/C2004A04997/2024-07-01/2024-07-01/text/1/epub/OEBPS/document_1/document_1.html#_Toc172806555> ;
    dcat:landingPage "https://www.legislation.gov.au/C2004A04997/2024-07-01/2024-07-01/text/1/epub/OEBPS/document_1/document_1.html#_Toc172806555"^^xsd:anyURI ;
    dcat:theme legcons:Item .

C2004A04997:57 a legcons:Item,
        C2004A04997:Item,
        owl:Class,
        dcat:Resource ;
    rdfs:label "Item - I57 20 A  Regulations"@en-AU ;
    dct:isPartOf C2004A04997:56 ;
    rdfs:comment "20 A  Regulations - Abrievated Graph Key: I57"@en-AU ;
    rdfs:subClassOf C2004A04997: ;
    skos:definition "20 A  Regulations"@en-AU ;
    skos:narrower C2004A04997:56 ;
    skos:prefLabel "Item I57"@en-AU ;
    dcat:accessURL <https://www.legislation.gov.au/C2004A04997/2024-07-01/2024-07-01/text/1/epub/OEBPS/document_1/document_1.html#_Toc172806557> ;
    dcat:landingPage "https://www.legislation.gov.au/C2004A04997/2024-07-01/2024-07-01/text/1/epub/OEBPS/document_1/document_1.html#_Toc172806557"^^xsd:anyURI ;
    dcat:theme legcons:Item .

C2004A04997:58 a legcons:Item,
        C2004A04997:Item,
        owl:Class,
        dcat:Resource ;
    rdfs:label "Item - I58 21  Repeal of the Customs Tariff Act 1987 etc"@en-AU ;
    dct:isPartOf C2004A04997:56 ;
    rdfs:comment "21  Repeal of the Customs Tariff Act 1987 etc - Abrievated Graph Key: I58"@en-AU ;
    rdfs:subClassOf C2004A04997: ;
    skos:definition "21  Repeal of the Customs Tariff Act 1987 etc"@en-AU ;
    skos:narrower C2004A04997:56 ;
    skos:prefLabel "Item I58"@en-AU ;
    dcat:accessURL <https://www.legislation.gov.au/C2004A04997/2024-07-01/2024-07-01/text/1/epub/OEBPS/document_1/document_1.html#_Toc172806558> ;
    dcat:landingPage "https://www.legislation.gov.au/C2004A04997/2024-07-01/2024-07-01/text/1/epub/OEBPS/document_1/document_1.html#_Toc172806558"^^xsd:anyURI ;
    dcat:theme legcons:Item .

C2004A04997:59 a legcons:Item,
        C2004A04997:Item,
        owl:Class,
        dcat:Resource ;
    rdfs:label "Item - I59 22  Transitional"@en-AU ;
    dct:isPartOf C2004A04997:56 ;
    rdfs:comment "22  Transitional - Abrievated Graph Key: I59"@en-AU ;
    rdfs:subClassOf C2004A04997: ;
    skos:definition "22  Transitional"@en-AU ;
    skos:narrower C2004A04997:56 ;
    skos:prefLabel "Item I59"@en-AU ;
    dcat:accessURL <https://www.legislation.gov.au/C2004A04997/2024-07-01/2024-07-01/text/1/epub/OEBPS/document_1/document_1.html#_Toc172806559> ;
    dcat:landingPage "https://www.legislation.gov.au/C2004A04997/2024-07-01/2024-07-01/text/1/epub/OEBPS/document_1/document_1.html#_Toc172806559"^^xsd:anyURI ;
    dcat:theme legcons:Item .

C2004A04997:6 a legcons:Item,
        C2004A04997:Item,
        owl:Class,
        dcat:Resource ;
    rdfs:label "Item - I6 3 A  Act does not extend to Norfolk Island"@en-AU ;
    dct:isPartOf C2004A04997:2 ;
    rdfs:comment "3 A  Act does not extend to Norfolk Island - Abrievated Graph Key: I6"@en-AU ;
    rdfs:subClassOf C2004A04997: ;
    skos:definition "3 A  Act does not extend to Norfolk Island"@en-AU ;
    skos:narrower C2004A04997:2 ;
    skos:prefLabel "Item I6"@en-AU ;
    dcat:accessURL <https://www.legislation.gov.au/C2004A04997/2024-07-01/2024-07-01/text/1/epub/OEBPS/document_1/document_1.html#_Toc172806506> ;
    dcat:landingPage "https://www.legislation.gov.au/C2004A04997/2024-07-01/2024-07-01/text/1/epub/OEBPS/document_1/document_1.html#_Toc172806506"^^xsd:anyURI ;
    dcat:theme legcons:Item .

C2004A04997:60 a legcons:Schedule,
        C2004A04997:Schedule,
        owl:Class,
        dcat:Resource ;
    rdfs:label "Schedule - S60 Schedule 2 General rules for the interpretation of Schedule 3"@en-AU ;
    dct:isPartOf C2004A04997:1 ;
    rdfs:comment "Schedule 2 General rules for the interpretation of Schedule 3 - Abrievated Graph Key: S60"@en-AU ;
    rdfs:subClassOf C2004A04997: ;
    skos:definition "Schedule 2 General rules for the interpretation of Schedule 3"@en-AU ;
    skos:narrower C2004A04997:1 ;
    skos:prefLabel "Schedule S60"@en-AU ;
    dcat:accessURL <https://www.legislation.gov.au/C2004A04997/2024-07-01/2024-07-01/text/1/epub/OEBPS/document_1/document_1.html#_Toc172806560> ;
    dcat:landingPage "https://www.legislation.gov.au/C2004A04997/2024-07-01/2024-07-01/text/1/epub/OEBPS/document_1/document_1.html#_Toc172806560"^^xsd:anyURI ;
    dcat:theme legcons:Schedule .

C2004A04997:63 a legcons:Item,
        C2004A04997:Item,
        owl:Class,
        dcat:Resource ;
    rdfs:label "Item - I63 Notes"@en-AU ;
    dct:isPartOf C2004A04997:62 ;
    rdfs:comment "Notes - Abrievated Graph Key: I63"@en-AU ;
    rdfs:subClassOf C2004A04997: ;
    skos:definition "Notes"@en-AU ;
    skos:narrower C2004A04997:62 ;
    skos:prefLabel "Item I63"@en-AU ;
    dcat:accessURL <https://www.legislation.gov.au/C2004A04997/2024-07-01/2024-07-01/text/1/epub/OEBPS/document_1/document_1.html#_Toc172806563> ;
    dcat:landingPage "https://www.legislation.gov.au/C2004A04997/2024-07-01/2024-07-01/text/1/epub/OEBPS/document_1/document_1.html#_Toc172806563"^^xsd:anyURI ;
    dcat:theme legcons:Item .

C2004A04997:64 a legcons:Chapter,
        C2004A04997:Chapter,
        owl:Class,
        dcat:Resource ;
    rdfs:label "Chapter - C64 Chapter 1 Live animals"@en-AU ;
    dct:isPartOf C2004A04997:62 ;
    rdfs:comment "Chapter 1 Live animals - Abrievated Graph Key: C64"@en-AU ;
    rdfs:subClassOf C2004A04997: ;
    skos:definition "Chapter 1 Live animals"@en-AU ;
    skos:narrower C2004A04997:62 ;
    skos:prefLabel "Chapter C64"@en-AU ;
    dcat:accessURL <https://www.legislation.gov.au/C2004A04997/2024-07-01/2024-07-01/text/1/epub/OEBPS/document_1/document_1.html#_Toc172806564> ;
    dcat:landingPage "https://www.legislation.gov.au/C2004A04997/2024-07-01/2024-07-01/text/1/epub/OEBPS/document_1/document_1.html#_Toc172806564"^^xsd:anyURI ;
    dcat:theme legcons:Chapter .

C2004A04997:65 a legcons:Item,
        C2004A04997:Item,
        owl:Class,
        dcat:Resource ;
    rdfs:label "Item - I65 Note"@en-AU ;
    dct:isPartOf C2004A04997:62 ;
    rdfs:comment "Note - Abrievated Graph Key: I65"@en-AU ;
    rdfs:subClassOf C2004A04997: ;
    skos:definition "Note"@en-AU ;
    skos:narrower C2004A04997:62 ;
    skos:prefLabel "Item I65"@en-AU ;
    dcat:accessURL <https://www.legislation.gov.au/C2004A04997/2024-07-01/2024-07-01/text/1/epub/OEBPS/document_1/document_1.html#_Toc172806565> ;
    dcat:landingPage "https://www.legislation.gov.au/C2004A04997/2024-07-01/2024-07-01/text/1/epub/OEBPS/document_1/document_1.html#_Toc172806565"^^xsd:anyURI ;
    dcat:theme legcons:Item .

C2004A04997:66 a legcons:Chapter,
        C2004A04997:Chapter,
        owl:Class,
        dcat:Resource ;
    rdfs:label "Chapter - C66 Chapter 2 Meat and edible meat offal"@en-AU ;
    dct:isPartOf C2004A04997:62 ;
    rdfs:comment "Chapter 2 Meat and edible meat offal - Abrievated Graph Key: C66"@en-AU ;
    rdfs:subClassOf C2004A04997: ;
    skos:definition "Chapter 2 Meat and edible meat offal"@en-AU ;
    skos:narrower C2004A04997:62 ;
    skos:prefLabel "Chapter C66"@en-AU ;
    dcat:accessURL <https://www.legislation.gov.au/C2004A04997/2024-07-01/2024-07-01/text/1/epub/OEBPS/document_1/document_1.html#_Toc172806566> ;
    dcat:landingPage "https://www.legislation.gov.au/C2004A04997/2024-07-01/2024-07-01/text/1/epub/OEBPS/document_1/document_1.html#_Toc172806566"^^xsd:anyURI ;
    dcat:theme legcons:Chapter .

C2004A04997:67 a legcons:Item,
        C2004A04997:Item,
        owl:Class,
        dcat:Resource ;
    rdfs:label "Item - I67 Note"@en-AU ;
    dct:isPartOf C2004A04997:62 ;
    rdfs:comment "Note - Abrievated Graph Key: I67"@en-AU ;
    rdfs:subClassOf C2004A04997: ;
    skos:definition "Note"@en-AU ;
    skos:narrower C2004A04997:62 ;
    skos:prefLabel "Item I67"@en-AU ;
    dcat:accessURL <https://www.legislation.gov.au/C2004A04997/2024-07-01/2024-07-01/text/1/epub/OEBPS/document_1/document_1.html#_Toc172806567> ;
    dcat:landingPage "https://www.legislation.gov.au/C2004A04997/2024-07-01/2024-07-01/text/1/epub/OEBPS/document_1/document_1.html#_Toc172806567"^^xsd:anyURI ;
    dcat:theme legcons:Item .

C2004A04997:68 a legcons:Chapter,
        C2004A04997:Chapter,
        owl:Class,
        dcat:Resource ;
    rdfs:label "Chapter - C68 Chapter 3 Fish and crustaceans molluscs and other aquatic invertebrates"@en-AU ;
    dct:isPartOf C2004A04997:62 ;
    rdfs:comment "Chapter 3 Fish and crustaceans molluscs and other aquatic invertebrates - Abrievated Graph Key: C68"@en-AU ;
    rdfs:subClassOf C2004A04997: ;
    skos:definition "Chapter 3 Fish and crustaceans molluscs and other aquatic invertebrates"@en-AU ;
    skos:narrower C2004A04997:62 ;
    skos:prefLabel "Chapter C68"@en-AU ;
    dcat:accessURL <https://www.legislation.gov.au/C2004A04997/2024-07-01/2024-07-01/text/1/epub/OEBPS/document_1/document_1.html#_Toc172806568> ;
    dcat:landingPage "https://www.legislation.gov.au/C2004A04997/2024-07-01/2024-07-01/text/1/epub/OEBPS/document_1/document_1.html#_Toc172806568"^^xsd:anyURI ;
    dcat:theme legcons:Chapter .

C2004A04997:69 a legcons:Item,
        C2004A04997:Item,
        owl:Class,
        dcat:Resource ;
    rdfs:label "Item - I69 Notes"@en-AU ;
    dct:isPartOf C2004A04997:62 ;
    rdfs:comment "Notes - Abrievated Graph Key: I69"@en-AU ;
    rdfs:subClassOf C2004A04997: ;
    skos:definition "Notes"@en-AU ;
    skos:narrower C2004A04997:62 ;
    skos:prefLabel "Item I69"@en-AU ;
    dcat:accessURL <https://www.legislation.gov.au/C2004A04997/2024-07-01/2024-07-01/text/1/epub/OEBPS/document_1/document_1.html#_Toc172806569> ;
    dcat:landingPage "https://www.legislation.gov.au/C2004A04997/2024-07-01/2024-07-01/text/1/epub/OEBPS/document_1/document_1.html#_Toc172806569"^^xsd:anyURI ;
    dcat:theme legcons:Item .

C2004A04997:7 a legcons:Item,
        C2004A04997:Item,
        owl:Class,
        dcat:Resource ;
    rdfs:label "Item - I7 4  Headings in Schedule 3"@en-AU ;
    dct:isPartOf C2004A04997:2 ;
    rdfs:comment "4  Headings in Schedule 3 - Abrievated Graph Key: I7"@en-AU ;
    rdfs:subClassOf C2004A04997: ;
    skos:definition "4  Headings in Schedule 3"@en-AU ;
    skos:narrower C2004A04997:2 ;
    skos:prefLabel "Item I7"@en-AU ;
    dcat:accessURL <https://www.legislation.gov.au/C2004A04997/2024-07-01/2024-07-01/text/1/epub/OEBPS/document_1/document_1.html#_Toc172806507> ;
    dcat:landingPage "https://www.legislation.gov.au/C2004A04997/2024-07-01/2024-07-01/text/1/epub/OEBPS/document_1/document_1.html#_Toc172806507"^^xsd:anyURI ;
    dcat:theme legcons:Item .

C2004A04997:70 a legcons:Chapter,
        C2004A04997:Chapter,
        owl:Class,
        dcat:Resource ;
    rdfs:label "Chapter - C70 Chapter 4 Dairy produce birds eggs natural honey edible products of animal origin not elsewhere specified or included"@en-AU ;
    dct:isPartOf C2004A04997:62 ;
    rdfs:comment "Chapter 4 Dairy produce birds eggs natural honey edible products of animal origin not elsewhere specified or included - Abrievated Graph Key: C70"@en-AU ;
    rdfs:subClassOf C2004A04997: ;
    skos:definition "Chapter 4 Dairy produce birds eggs natural honey edible products of animal origin not elsewhere specified or included"@en-AU ;
    skos:narrower C2004A04997:62 ;
    skos:prefLabel "Chapter C70"@en-AU ;
    dcat:accessURL <https://www.legislation.gov.au/C2004A04997/2024-07-01/2024-07-01/text/1/epub/OEBPS/document_1/document_1.html#_Toc172806570> ;
    dcat:landingPage "https://www.legislation.gov.au/C2004A04997/2024-07-01/2024-07-01/text/1/epub/OEBPS/document_1/document_1.html#_Toc172806570"^^xsd:anyURI ;
    dcat:theme legcons:Chapter .

C2004A04997:71 a legcons:Item,
        C2004A04997:Item,
        owl:Class,
        dcat:Resource ;
    rdfs:label "Item - I71 Notes"@en-AU ;
    dct:isPartOf C2004A04997:62 ;
    rdfs:comment "Notes - Abrievated Graph Key: I71"@en-AU ;
    rdfs:subClassOf C2004A04997: ;
    skos:definition "Notes"@en-AU ;
    skos:narrower C2004A04997:62 ;
    skos:prefLabel "Item I71"@en-AU ;
    dcat:accessURL <https://www.legislation.gov.au/C2004A04997/2024-07-01/2024-07-01/text/1/epub/OEBPS/document_1/document_1.html#_Toc172806571> ;
    dcat:landingPage "https://www.legislation.gov.au/C2004A04997/2024-07-01/2024-07-01/text/1/epub/OEBPS/document_1/document_1.html#_Toc172806571"^^xsd:anyURI ;
    dcat:theme legcons:Item .

C2004A04997:72 a legcons:Item,
        C2004A04997:Item,
        owl:Class,
        dcat:Resource ;
    rdfs:label "Item - I72 Subheading Notes"@en-AU ;
    dct:isPartOf C2004A04997:62 ;
    rdfs:comment "Subheading Notes - Abrievated Graph Key: I72"@en-AU ;
    rdfs:subClassOf C2004A04997: ;
    skos:definition "Subheading Notes"@en-AU ;
    skos:narrower C2004A04997:62 ;
    skos:prefLabel "Item I72"@en-AU ;
    dcat:accessURL <https://www.legislation.gov.au/C2004A04997/2024-07-01/2024-07-01/text/1/epub/OEBPS/document_1/document_1.html#_Toc172806572> ;
    dcat:landingPage "https://www.legislation.gov.au/C2004A04997/2024-07-01/2024-07-01/text/1/epub/OEBPS/document_1/document_1.html#_Toc172806572"^^xsd:anyURI ;
    dcat:theme legcons:Item .

C2004A04997:73 a legcons:Chapter,
        C2004A04997:Chapter,
        owl:Class,
        dcat:Resource ;
    rdfs:label "Chapter - C73 Chapter 5 Products of animal origin not elsewhere specified or included"@en-AU ;
    dct:isPartOf C2004A04997:62 ;
    rdfs:comment "Chapter 5 Products of animal origin not elsewhere specified or included - Abrievated Graph Key: C73"@en-AU ;
    rdfs:subClassOf C2004A04997: ;
    skos:definition "Chapter 5 Products of animal origin not elsewhere specified or included"@en-AU ;
    skos:narrower C2004A04997:62 ;
    skos:prefLabel "Chapter C73"@en-AU ;
    dcat:accessURL <https://www.legislation.gov.au/C2004A04997/2024-07-01/2024-07-01/text/1/epub/OEBPS/document_1/document_1.html#_Toc172806573> ;
    dcat:landingPage "https://www.legislation.gov.au/C2004A04997/2024-07-01/2024-07-01/text/1/epub/OEBPS/document_1/document_1.html#_Toc172806573"^^xsd:anyURI ;
    dcat:theme legcons:Chapter .

C2004A04997:74 a legcons:Item,
        C2004A04997:Item,
        owl:Class,
        dcat:Resource ;
    rdfs:label "Item - I74 Notes"@en-AU ;
    dct:isPartOf C2004A04997:62 ;
    rdfs:comment "Notes - Abrievated Graph Key: I74"@en-AU ;
    rdfs:subClassOf C2004A04997: ;
    skos:definition "Notes"@en-AU ;
    skos:narrower C2004A04997:62 ;
    skos:prefLabel "Item I74"@en-AU ;
    dcat:accessURL <https://www.legislation.gov.au/C2004A04997/2024-07-01/2024-07-01/text/1/epub/OEBPS/document_1/document_1.html#_Toc172806574> ;
    dcat:landingPage "https://www.legislation.gov.au/C2004A04997/2024-07-01/2024-07-01/text/1/epub/OEBPS/document_1/document_1.html#_Toc172806574"^^xsd:anyURI ;
    dcat:theme legcons:Item .

C2004A04997:75 a legcons:Section,
        C2004A04997:Section,
        owl:Class,
        dcat:Resource ;
    rdfs:label "Section - S75 Section IIVegetable products"@en-AU ;
    dct:isPartOf C2004A04997:61 ;
    rdfs:comment "Section IIVegetable products - Abrievated Graph Key: S75"@en-AU ;
    rdfs:subClassOf C2004A04997: ;
    skos:definition "Section IIVegetable products"@en-AU ;
    skos:narrower C2004A04997:61 ;
    skos:prefLabel "Section S75"@en-AU ;
    dcat:accessURL <https://www.legislation.gov.au/C2004A04997/2024-07-01/2024-07-01/text/1/epub/OEBPS/document_1/document_1.html#_Toc172806575> ;
    dcat:landingPage "https://www.legislation.gov.au/C2004A04997/2024-07-01/2024-07-01/text/1/epub/OEBPS/document_1/document_1.html#_Toc172806575"^^xsd:anyURI ;
    dcat:theme legcons:Section .

C2004A04997:76 a legcons:Item,
        C2004A04997:Item,
        owl:Class,
        dcat:Resource ;
    rdfs:label "Item - I76 Note"@en-AU ;
    dct:isPartOf C2004A04997:61 ;
    rdfs:comment "Note - Abrievated Graph Key: I76"@en-AU ;
    rdfs:subClassOf C2004A04997: ;
    skos:definition "Note"@en-AU ;
    skos:narrower C2004A04997:61 ;
    skos:prefLabel "Item I76"@en-AU ;
    dcat:accessURL <https://www.legislation.gov.au/C2004A04997/2024-07-01/2024-07-01/text/1/epub/OEBPS/document_1/document_1.html#_Toc172806576> ;
    dcat:landingPage "https://www.legislation.gov.au/C2004A04997/2024-07-01/2024-07-01/text/1/epub/OEBPS/document_1/document_1.html#_Toc172806576"^^xsd:anyURI ;
    dcat:theme legcons:Item .

C2004A04997:77 a legcons:Chapter,
        C2004A04997:Chapter,
        owl:Class,
        dcat:Resource ;
    rdfs:label "Chapter - C77 Chapter 6 Live trees and other plants bulbs roots and the like cut flowers and ornamental foliage"@en-AU ;
    dct:isPartOf C2004A04997:61 ;
    rdfs:comment "Chapter 6 Live trees and other plants bulbs roots and the like cut flowers and ornamental foliage - Abrievated Graph Key: C77"@en-AU ;
    rdfs:subClassOf C2004A04997: ;
    skos:definition "Chapter 6 Live trees and other plants bulbs roots and the like cut flowers and ornamental foliage"@en-AU ;
    skos:narrower C2004A04997:61 ;
    skos:prefLabel "Chapter C77"@en-AU ;
    dcat:accessURL <https://www.legislation.gov.au/C2004A04997/2024-07-01/2024-07-01/text/1/epub/OEBPS/document_1/document_1.html#_Toc172806577> ;
    dcat:landingPage "https://www.legislation.gov.au/C2004A04997/2024-07-01/2024-07-01/text/1/epub/OEBPS/document_1/document_1.html#_Toc172806577"^^xsd:anyURI ;
    dcat:theme legcons:Chapter .

C2004A04997:78 a legcons:Item,
        C2004A04997:Item,
        owl:Class,
        dcat:Resource ;
    rdfs:label "Item - I78 Notes"@en-AU ;
    dct:isPartOf C2004A04997:61 ;
    rdfs:comment "Notes - Abrievated Graph Key: I78"@en-AU ;
    rdfs:subClassOf C2004A04997: ;
    skos:definition "Notes"@en-AU ;
    skos:narrower C2004A04997:61 ;
    skos:prefLabel "Item I78"@en-AU ;
    dcat:accessURL <https://www.legislation.gov.au/C2004A04997/2024-07-01/2024-07-01/text/1/epub/OEBPS/document_1/document_1.html#_Toc172806578> ;
    dcat:landingPage "https://www.legislation.gov.au/C2004A04997/2024-07-01/2024-07-01/text/1/epub/OEBPS/document_1/document_1.html#_Toc172806578"^^xsd:anyURI ;
    dcat:theme legcons:Item .

C2004A04997:79 a legcons:Chapter,
        C2004A04997:Chapter,
        owl:Class,
        dcat:Resource ;
    rdfs:label "Chapter - C79 Chapter 7 Edible vegetables and certain roots and tubers"@en-AU ;
    dct:isPartOf C2004A04997:61 ;
    rdfs:comment "Chapter 7 Edible vegetables and certain roots and tubers - Abrievated Graph Key: C79"@en-AU ;
    rdfs:subClassOf C2004A04997: ;
    skos:definition "Chapter 7 Edible vegetables and certain roots and tubers"@en-AU ;
    skos:narrower C2004A04997:61 ;
    skos:prefLabel "Chapter C79"@en-AU ;
    dcat:accessURL <https://www.legislation.gov.au/C2004A04997/2024-07-01/2024-07-01/text/1/epub/OEBPS/document_1/document_1.html#_Toc172806579> ;
    dcat:landingPage "https://www.legislation.gov.au/C2004A04997/2024-07-01/2024-07-01/text/1/epub/OEBPS/document_1/document_1.html#_Toc172806579"^^xsd:anyURI ;
    dcat:theme legcons:Chapter .

C2004A04997:8 a legcons:Item,
        C2004A04997:Item,
        owl:Class,
        dcat:Resource ;
    rdfs:label "Item - I8 5  Items in Schedule 4"@en-AU ;
    dct:isPartOf C2004A04997:2 ;
    rdfs:comment "5  Items in Schedule 4 - Abrievated Graph Key: I8"@en-AU ;
    rdfs:subClassOf C2004A04997: ;
    skos:definition "5  Items in Schedule 4"@en-AU ;
    skos:narrower C2004A04997:2 ;
    skos:prefLabel "Item I8"@en-AU ;
    dcat:accessURL <https://www.legislation.gov.au/C2004A04997/2024-07-01/2024-07-01/text/1/epub/OEBPS/document_1/document_1.html#_Toc172806508> ;
    dcat:landingPage "https://www.legislation.gov.au/C2004A04997/2024-07-01/2024-07-01/text/1/epub/OEBPS/document_1/document_1.html#_Toc172806508"^^xsd:anyURI ;
    dcat:theme legcons:Item .

C2004A04997:80 a legcons:Item,
        C2004A04997:Item,
        owl:Class,
        dcat:Resource ;
    rdfs:label "Item - I80 Notes"@en-AU ;
    dct:isPartOf C2004A04997:61 ;
    rdfs:comment "Notes - Abrievated Graph Key: I80"@en-AU ;
    rdfs:subClassOf C2004A04997: ;
    skos:definition "Notes"@en-AU ;
    skos:narrower C2004A04997:61 ;
    skos:prefLabel "Item I80"@en-AU ;
    dcat:accessURL <https://www.legislation.gov.au/C2004A04997/2024-07-01/2024-07-01/text/1/epub/OEBPS/document_1/document_1.html#_Toc172806580> ;
    dcat:landingPage "https://www.legislation.gov.au/C2004A04997/2024-07-01/2024-07-01/text/1/epub/OEBPS/document_1/document_1.html#_Toc172806580"^^xsd:anyURI ;
    dcat:theme legcons:Item .

C2004A04997:81 a legcons:Chapter,
        C2004A04997:Chapter,
        owl:Class,
        dcat:Resource ;
    rdfs:label "Chapter - C81 Chapter 8 Edible fruit and nuts peel of citrus fruit or melons"@en-AU ;
    dct:isPartOf C2004A04997:61 ;
    rdfs:comment "Chapter 8 Edible fruit and nuts peel of citrus fruit or melons - Abrievated Graph Key: C81"@en-AU ;
    rdfs:subClassOf C2004A04997: ;
    skos:definition "Chapter 8 Edible fruit and nuts peel of citrus fruit or melons"@en-AU ;
    skos:narrower C2004A04997:61 ;
    skos:prefLabel "Chapter C81"@en-AU ;
    dcat:accessURL <https://www.legislation.gov.au/C2004A04997/2024-07-01/2024-07-01/text/1/epub/OEBPS/document_1/document_1.html#_Toc172806581> ;
    dcat:landingPage "https://www.legislation.gov.au/C2004A04997/2024-07-01/2024-07-01/text/1/epub/OEBPS/document_1/document_1.html#_Toc172806581"^^xsd:anyURI ;
    dcat:theme legcons:Chapter .

C2004A04997:82 a legcons:Item,
        C2004A04997:Item,
        owl:Class,
        dcat:Resource ;
    rdfs:label "Item - I82 Notes"@en-AU ;
    dct:isPartOf C2004A04997:61 ;
    rdfs:comment "Notes - Abrievated Graph Key: I82"@en-AU ;
    rdfs:subClassOf C2004A04997: ;
    skos:definition "Notes"@en-AU ;
    skos:narrower C2004A04997:61 ;
    skos:prefLabel "Item I82"@en-AU ;
    dcat:accessURL <https://www.legislation.gov.au/C2004A04997/2024-07-01/2024-07-01/text/1/epub/OEBPS/document_1/document_1.html#_Toc172806582> ;
    dcat:landingPage "https://www.legislation.gov.au/C2004A04997/2024-07-01/2024-07-01/text/1/epub/OEBPS/document_1/document_1.html#_Toc172806582"^^xsd:anyURI ;
    dcat:theme legcons:Item .

C2004A04997:83 a legcons:Chapter,
        C2004A04997:Chapter,
        owl:Class,
        dcat:Resource ;
    rdfs:label "Chapter - C83 Chapter 9 Coffee tea mate and spices"@en-AU ;
    dct:isPartOf C2004A04997:61 ;
    rdfs:comment "Chapter 9 Coffee tea mate and spices - Abrievated Graph Key: C83"@en-AU ;
    rdfs:subClassOf C2004A04997: ;
    skos:definition "Chapter 9 Coffee tea mate and spices"@en-AU ;
    skos:narrower C2004A04997:61 ;
    skos:prefLabel "Chapter C83"@en-AU ;
    dcat:accessURL <https://www.legislation.gov.au/C2004A04997/2024-07-01/2024-07-01/text/1/epub/OEBPS/document_1/document_1.html#_Toc172806583> ;
    dcat:landingPage "https://www.legislation.gov.au/C2004A04997/2024-07-01/2024-07-01/text/1/epub/OEBPS/document_1/document_1.html#_Toc172806583"^^xsd:anyURI ;
    dcat:theme legcons:Chapter .

C2004A04997:84 a legcons:Item,
        C2004A04997:Item,
        owl:Class,
        dcat:Resource ;
    rdfs:label "Item - I84 Notes"@en-AU ;
    dct:isPartOf C2004A04997:61 ;
    rdfs:comment "Notes - Abrievated Graph Key: I84"@en-AU ;
    rdfs:subClassOf C2004A04997: ;
    skos:definition "Notes"@en-AU ;
    skos:narrower C2004A04997:61 ;
    skos:prefLabel "Item I84"@en-AU ;
    dcat:accessURL <https://www.legislation.gov.au/C2004A04997/2024-07-01/2024-07-01/text/1/epub/OEBPS/document_1/document_1.html#_Toc172806584> ;
    dcat:landingPage "https://www.legislation.gov.au/C2004A04997/2024-07-01/2024-07-01/text/1/epub/OEBPS/document_1/document_1.html#_Toc172806584"^^xsd:anyURI ;
    dcat:theme legcons:Item .

C2004A04997:85 a legcons:Chapter,
        C2004A04997:Chapter,
        owl:Class,
        dcat:Resource ;
    rdfs:label "Chapter - C85 Chapter 10 Cereals"@en-AU ;
    dct:isPartOf C2004A04997:61 ;
    rdfs:comment "Chapter 10 Cereals - Abrievated Graph Key: C85"@en-AU ;
    rdfs:subClassOf C2004A04997: ;
    skos:definition "Chapter 10 Cereals"@en-AU ;
    skos:narrower C2004A04997:61 ;
    skos:prefLabel "Chapter C85"@en-AU ;
    dcat:accessURL <https://www.legislation.gov.au/C2004A04997/2024-07-01/2024-07-01/text/1/epub/OEBPS/document_1/document_1.html#_Toc172806585> ;
    dcat:landingPage "https://www.legislation.gov.au/C2004A04997/2024-07-01/2024-07-01/text/1/epub/OEBPS/document_1/document_1.html#_Toc172806585"^^xsd:anyURI ;
    dcat:theme legcons:Chapter .

C2004A04997:86 a legcons:Item,
        C2004A04997:Item,
        owl:Class,
        dcat:Resource ;
    rdfs:label "Item - I86 Notes"@en-AU ;
    dct:isPartOf C2004A04997:61 ;
    rdfs:comment "Notes - Abrievated Graph Key: I86"@en-AU ;
    rdfs:subClassOf C2004A04997: ;
    skos:definition "Notes"@en-AU ;
    skos:narrower C2004A04997:61 ;
    skos:prefLabel "Item I86"@en-AU ;
    dcat:accessURL <https://www.legislation.gov.au/C2004A04997/2024-07-01/2024-07-01/text/1/epub/OEBPS/document_1/document_1.html#_Toc172806586> ;
    dcat:landingPage "https://www.legislation.gov.au/C2004A04997/2024-07-01/2024-07-01/text/1/epub/OEBPS/document_1/document_1.html#_Toc172806586"^^xsd:anyURI ;
    dcat:theme legcons:Item .

C2004A04997:87 a legcons:Item,
        C2004A04997:Item,
        owl:Class,
        dcat:Resource ;
    rdfs:label "Item - I87 Subheading Note"@en-AU ;
    dct:isPartOf C2004A04997:61 ;
    rdfs:comment "Subheading Note - Abrievated Graph Key: I87"@en-AU ;
    rdfs:subClassOf C2004A04997: ;
    skos:definition "Subheading Note"@en-AU ;
    skos:narrower C2004A04997:61 ;
    skos:prefLabel "Item I87"@en-AU ;
    dcat:accessURL <https://www.legislation.gov.au/C2004A04997/2024-07-01/2024-07-01/text/1/epub/OEBPS/document_1/document_1.html#_Toc172806587> ;
    dcat:landingPage "https://www.legislation.gov.au/C2004A04997/2024-07-01/2024-07-01/text/1/epub/OEBPS/document_1/document_1.html#_Toc172806587"^^xsd:anyURI ;
    dcat:theme legcons:Item .

C2004A04997:88 a legcons:Chapter,
        C2004A04997:Chapter,
        owl:Class,
        dcat:Resource ;
    rdfs:label "Chapter - C88 Chapter 11 Products of the milling industry malt starches inulin wheat gluten"@en-AU ;
    dct:isPartOf C2004A04997:61 ;
    rdfs:comment "Chapter 11 Products of the milling industry malt starches inulin wheat gluten - Abrievated Graph Key: C88"@en-AU ;
    rdfs:subClassOf C2004A04997: ;
    skos:definition "Chapter 11 Products of the milling industry malt starches inulin wheat gluten"@en-AU ;
    skos:narrower C2004A04997:61 ;
    skos:prefLabel "Chapter C88"@en-AU ;
    dcat:accessURL <https://www.legislation.gov.au/C2004A04997/2024-07-01/2024-07-01/text/1/epub/OEBPS/document_1/document_1.html#_Toc172806588> ;
    dcat:landingPage "https://www.legislation.gov.au/C2004A04997/2024-07-01/2024-07-01/text/1/epub/OEBPS/document_1/document_1.html#_Toc172806588"^^xsd:anyURI ;
    dcat:theme legcons:Chapter .

C2004A04997:89 a legcons:Item,
        C2004A04997:Item,
        owl:Class,
        dcat:Resource ;
    rdfs:label "Item - I89 Notes"@en-AU ;
    dct:isPartOf C2004A04997:61 ;
    rdfs:comment "Notes - Abrievated Graph Key: I89"@en-AU ;
    rdfs:subClassOf C2004A04997: ;
    skos:definition "Notes"@en-AU ;
    skos:narrower C2004A04997:61 ;
    skos:prefLabel "Item I89"@en-AU ;
    dcat:accessURL <https://www.legislation.gov.au/C2004A04997/2024-07-01/2024-07-01/text/1/epub/OEBPS/document_1/document_1.html#_Toc172806589> ;
    dcat:landingPage "https://www.legislation.gov.au/C2004A04997/2024-07-01/2024-07-01/text/1/epub/OEBPS/document_1/document_1.html#_Toc172806589"^^xsd:anyURI ;
    dcat:theme legcons:Item .

C2004A04997:9 a legcons:Item,
        C2004A04997:Item,
        owl:Class,
        dcat:Resource ;
    rdfs:label "Item - I9 6  Tariff classification"@en-AU ;
    dct:isPartOf C2004A04997:2 ;
    rdfs:comment "6  Tariff classification - Abrievated Graph Key: I9"@en-AU ;
    rdfs:subClassOf C2004A04997: ;
    skos:definition "6  Tariff classification"@en-AU ;
    skos:narrower C2004A04997:2 ;
    skos:prefLabel "Item I9"@en-AU ;
    dcat:accessURL <https://www.legislation.gov.au/C2004A04997/2024-07-01/2024-07-01/text/1/epub/OEBPS/document_1/document_1.html#_Toc172806509> ;
    dcat:landingPage "https://www.legislation.gov.au/C2004A04997/2024-07-01/2024-07-01/text/1/epub/OEBPS/document_1/document_1.html#_Toc172806509"^^xsd:anyURI ;
    dcat:theme legcons:Item .

C2004A04997:90 a legcons:Chapter,
        C2004A04997:Chapter,
        owl:Class,
        dcat:Resource ;
    rdfs:label "Chapter - C90 Chapter 12 Oil seeds and oleaginous fruits miscellaneous grains seeds and fruit industrial or medicinal plants straw and fodder"@en-AU ;
    dct:isPartOf C2004A04997:61 ;
    rdfs:comment "Chapter 12 Oil seeds and oleaginous fruits miscellaneous grains seeds and fruit industrial or medicinal plants straw and fodder - Abrievated Graph Key: C90"@en-AU ;
    rdfs:subClassOf C2004A04997: ;
    skos:definition "Chapter 12 Oil seeds and oleaginous fruits miscellaneous grains seeds and fruit industrial or medicinal plants straw and fodder"@en-AU ;
    skos:narrower C2004A04997:61 ;
    skos:prefLabel "Chapter C90"@en-AU ;
    dcat:accessURL <https://www.legislation.gov.au/C2004A04997/2024-07-01/2024-07-01/text/1/epub/OEBPS/document_1/document_1.html#_Toc172806590> ;
    dcat:landingPage "https://www.legislation.gov.au/C2004A04997/2024-07-01/2024-07-01/text/1/epub/OEBPS/document_1/document_1.html#_Toc172806590"^^xsd:anyURI ;
    dcat:theme legcons:Chapter .

C2004A04997:91 a legcons:Item,
        C2004A04997:Item,
        owl:Class,
        dcat:Resource ;
    rdfs:label "Item - I91 Notes"@en-AU ;
    dct:isPartOf C2004A04997:61 ;
    rdfs:comment "Notes - Abrievated Graph Key: I91"@en-AU ;
    rdfs:subClassOf C2004A04997: ;
    skos:definition "Notes"@en-AU ;
    skos:narrower C2004A04997:61 ;
    skos:prefLabel "Item I91"@en-AU ;
    dcat:accessURL <https://www.legislation.gov.au/C2004A04997/2024-07-01/2024-07-01/text/1/epub/OEBPS/document_1/document_1.html#_Toc172806591> ;
    dcat:landingPage "https://www.legislation.gov.au/C2004A04997/2024-07-01/2024-07-01/text/1/epub/OEBPS/document_1/document_1.html#_Toc172806591"^^xsd:anyURI ;
    dcat:theme legcons:Item .

C2004A04997:92 a legcons:Item,
        C2004A04997:Item,
        owl:Class,
        dcat:Resource ;
    rdfs:label "Item - I92 Subheading Note"@en-AU ;
    dct:isPartOf C2004A04997:61 ;
    rdfs:comment "Subheading Note - Abrievated Graph Key: I92"@en-AU ;
    rdfs:subClassOf C2004A04997: ;
    skos:definition "Subheading Note"@en-AU ;
    skos:narrower C2004A04997:61 ;
    skos:prefLabel "Item I92"@en-AU ;
    dcat:accessURL <https://www.legislation.gov.au/C2004A04997/2024-07-01/2024-07-01/text/1/epub/OEBPS/document_1/document_1.html#_Toc172806592> ;
    dcat:landingPage "https://www.legislation.gov.au/C2004A04997/2024-07-01/2024-07-01/text/1/epub/OEBPS/document_1/document_1.html#_Toc172806592"^^xsd:anyURI ;
    dcat:theme legcons:Item .

C2004A04997:93 a legcons:Chapter,
        C2004A04997:Chapter,
        owl:Class,
        dcat:Resource ;
    rdfs:label "Chapter - C93 Chapter 13 Lac gums resins and other vegetable saps and extracts"@en-AU ;
    dct:isPartOf C2004A04997:61 ;
    rdfs:comment "Chapter 13 Lac gums resins and other vegetable saps and extracts - Abrievated Graph Key: C93"@en-AU ;
    rdfs:subClassOf C2004A04997: ;
    skos:definition "Chapter 13 Lac gums resins and other vegetable saps and extracts"@en-AU ;
    skos:narrower C2004A04997:61 ;
    skos:prefLabel "Chapter C93"@en-AU ;
    dcat:accessURL <https://www.legislation.gov.au/C2004A04997/2024-07-01/2024-07-01/text/1/epub/OEBPS/document_1/document_1.html#_Toc172806593> ;
    dcat:landingPage "https://www.legislation.gov.au/C2004A04997/2024-07-01/2024-07-01/text/1/epub/OEBPS/document_1/document_1.html#_Toc172806593"^^xsd:anyURI ;
    dcat:theme legcons:Chapter .

C2004A04997:94 a legcons:Item,
        C2004A04997:Item,
        owl:Class,
        dcat:Resource ;
    rdfs:label "Item - I94 Note"@en-AU ;
    dct:isPartOf C2004A04997:61 ;
    rdfs:comment "Note - Abrievated Graph Key: I94"@en-AU ;
    rdfs:subClassOf C2004A04997: ;
    skos:definition "Note"@en-AU ;
    skos:narrower C2004A04997:61 ;
    skos:prefLabel "Item I94"@en-AU ;
    dcat:accessURL <https://www.legislation.gov.au/C2004A04997/2024-07-01/2024-07-01/text/1/epub/OEBPS/document_1/document_1.html#_Toc172806594> ;
    dcat:landingPage "https://www.legislation.gov.au/C2004A04997/2024-07-01/2024-07-01/text/1/epub/OEBPS/document_1/document_1.html#_Toc172806594"^^xsd:anyURI ;
    dcat:theme legcons:Item .

C2004A04997:95 a legcons:Chapter,
        C2004A04997:Chapter,
        owl:Class,
        dcat:Resource ;
    rdfs:label "Chapter - C95 Chapter 14 Vegetable plaiting materials vegetable products not elsewhere specified or included"@en-AU ;
    dct:isPartOf C2004A04997:61 ;
    rdfs:comment "Chapter 14 Vegetable plaiting materials vegetable products not elsewhere specified or included - Abrievated Graph Key: C95"@en-AU ;
    rdfs:subClassOf C2004A04997: ;
    skos:definition "Chapter 14 Vegetable plaiting materials vegetable products not elsewhere specified or included"@en-AU ;
    skos:narrower C2004A04997:61 ;
    skos:prefLabel "Chapter C95"@en-AU ;
    dcat:accessURL <https://www.legislation.gov.au/C2004A04997/2024-07-01/2024-07-01/text/1/epub/OEBPS/document_1/document_1.html#_Toc172806595> ;
    dcat:landingPage "https://www.legislation.gov.au/C2004A04997/2024-07-01/2024-07-01/text/1/epub/OEBPS/document_1/document_1.html#_Toc172806595"^^xsd:anyURI ;
    dcat:theme legcons:Chapter .

C2004A04997:96 a legcons:Item,
        C2004A04997:Item,
        owl:Class,
        dcat:Resource ;
    rdfs:label "Item - I96 Notes"@en-AU ;
    dct:isPartOf C2004A04997:61 ;
    rdfs:comment "Notes - Abrievated Graph Key: I96"@en-AU ;
    rdfs:subClassOf C2004A04997: ;
    skos:definition "Notes"@en-AU ;
    skos:narrower C2004A04997:61 ;
    skos:prefLabel "Item I96"@en-AU ;
    dcat:accessURL <https://www.legislation.gov.au/C2004A04997/2024-07-01/2024-07-01/text/1/epub/OEBPS/document_1/document_1.html#_Toc172806596> ;
    dcat:landingPage "https://www.legislation.gov.au/C2004A04997/2024-07-01/2024-07-01/text/1/epub/OEBPS/document_1/document_1.html#_Toc172806596"^^xsd:anyURI ;
    dcat:theme legcons:Item .

C2004A04997:97 a legcons:Section,
        C2004A04997:Section,
        owl:Class,
        dcat:Resource ;
    rdfs:label "Section - S97 Section IIIAnimal vegetable or microbial fats and oils and their cleavage products prepared edible fats animal or vegetable waxes"@en-AU ;
    dct:isPartOf C2004A04997:61 ;
    rdfs:comment "Section IIIAnimal vegetable or microbial fats and oils and their cleavage products prepared edible fats animal or vegetable waxes - Abrievated Graph Key: S97"@en-AU ;
    rdfs:subClassOf C2004A04997: ;
    skos:definition "Section IIIAnimal vegetable or microbial fats and oils and their cleavage products prepared edible fats animal or vegetable waxes"@en-AU ;
    skos:narrower C2004A04997:61 ;
    skos:prefLabel "Section S97"@en-AU ;
    dcat:accessURL <https://www.legislation.gov.au/C2004A04997/2024-07-01/2024-07-01/text/1/epub/OEBPS/document_1/document_1.html#_Toc172806597> ;
    dcat:landingPage "https://www.legislation.gov.au/C2004A04997/2024-07-01/2024-07-01/text/1/epub/OEBPS/document_1/document_1.html#_Toc172806597"^^xsd:anyURI ;
    dcat:theme legcons:Section .

C2004A04997:98 a legcons:Chapter,
        C2004A04997:Chapter,
        owl:Class,
        dcat:Resource ;
    rdfs:label "Chapter - C98 Chapter 15 Animal vegetable or microbial fats and oils and their cleavage products prepared edible fats animal or vegetable waxes"@en-AU ;
    dct:isPartOf C2004A04997:61 ;
    rdfs:comment "Chapter 15 Animal vegetable or microbial fats and oils and their cleavage products prepared edible fats animal or vegetable waxes - Abrievated Graph Key: C98"@en-AU ;
    rdfs:subClassOf C2004A04997: ;
    skos:definition "Chapter 15 Animal vegetable or microbial fats and oils and their cleavage products prepared edible fats animal or vegetable waxes"@en-AU ;
    skos:narrower C2004A04997:61 ;
    skos:prefLabel "Chapter C98"@en-AU ;
    dcat:accessURL <https://www.legislation.gov.au/C2004A04997/2024-07-01/2024-07-01/text/1/epub/OEBPS/document_1/document_1.html#_Toc172806598> ;
    dcat:landingPage "https://www.legislation.gov.au/C2004A04997/2024-07-01/2024-07-01/text/1/epub/OEBPS/document_1/document_1.html#_Toc172806598"^^xsd:anyURI ;
    dcat:theme legcons:Chapter .

C2004A04997:99 a legcons:Item,
        C2004A04997:Item,
        owl:Class,
        dcat:Resource ;
    rdfs:label "Item - I99 Notes"@en-AU ;
    dct:isPartOf C2004A04997:61 ;
    rdfs:comment "Notes - Abrievated Graph Key: I99"@en-AU ;
    rdfs:subClassOf C2004A04997: ;
    skos:definition "Notes"@en-AU ;
    skos:narrower C2004A04997:61 ;
    skos:prefLabel "Item I99"@en-AU ;
    dcat:accessURL <https://www.legislation.gov.au/C2004A04997/2024-07-01/2024-07-01/text/1/epub/OEBPS/document_1/document_1.html#_Toc172806599> ;
    dcat:landingPage "https://www.legislation.gov.au/C2004A04997/2024-07-01/2024-07-01/text/1/epub/OEBPS/document_1/document_1.html#_Toc172806599"^^xsd:anyURI ;
    dcat:theme legcons:Item .

C2004A04997:281 a legcons:Chapter,
        C2004A04997:Chapter,
        owl:Class,
        dcat:Resource ;
    rdfs:label "Chapter - C281 Chapter 65 Headgear and parts thereof"@en-AU ;
    dct:hasPart C2004A04997:282 ;
    dct:isPartOf C2004A04997:277 ;
    rdfs:comment "Chapter 65 Headgear and parts thereof - Abrievated Graph Key: C281"@en-AU ;
    rdfs:subClassOf C2004A04997: ;
    skos:broader C2004A04997:282 ;
    skos:definition "Chapter 65 Headgear and parts thereof"@en-AU ;
    skos:narrower C2004A04997:277 ;
    skos:prefLabel "Chapter C281"@en-AU ;
    dcat:accessURL <https://www.legislation.gov.au/C2004A04997/2024-07-01/2024-07-01/text/1/epub/OEBPS/document_4/document_4.html#_Toc171752012> ;
    dcat:landingPage "https://www.legislation.gov.au/C2004A04997/2024-07-01/2024-07-01/text/1/epub/OEBPS/document_4/document_4.html#_Toc171752012"^^xsd:anyURI ;
    dcat:theme legcons:Chapter .

C2004A04997:283 a legcons:Chapter,
        C2004A04997:Chapter,
        owl:Class,
        dcat:Resource ;
    rdfs:label "Chapter - C283 Chapter 66 Umbrellas sun umbrellas walking sticks seat sticks whips riding crops and parts thereof"@en-AU ;
    dct:hasPart C2004A04997:284 ;
    dct:isPartOf C2004A04997:277 ;
    rdfs:comment "Chapter 66 Umbrellas sun umbrellas walking sticks seat sticks whips riding crops and parts thereof - Abrievated Graph Key: C283"@en-AU ;
    rdfs:subClassOf C2004A04997: ;
    skos:broader C2004A04997:284 ;
    skos:definition "Chapter 66 Umbrellas sun umbrellas walking sticks seat sticks whips riding crops and parts thereof"@en-AU ;
    skos:narrower C2004A04997:277 ;
    skos:prefLabel "Chapter C283"@en-AU ;
    dcat:accessURL <https://www.legislation.gov.au/C2004A04997/2024-07-01/2024-07-01/text/1/epub/OEBPS/document_4/document_4.html#_Toc171752014> ;
    dcat:landingPage "https://www.legislation.gov.au/C2004A04997/2024-07-01/2024-07-01/text/1/epub/OEBPS/document_4/document_4.html#_Toc171752014"^^xsd:anyURI ;
    dcat:theme legcons:Chapter .

C2004A04997:285 a legcons:Chapter,
        C2004A04997:Chapter,
        owl:Class,
        dcat:Resource ;
    rdfs:label "Chapter - C285 Chapter 67 Prepared feathers and down and articles made of feathers or of down artificial flowers articles of human hair"@en-AU ;
    dct:hasPart C2004A04997:286 ;
    dct:isPartOf C2004A04997:277 ;
    rdfs:comment "Chapter 67 Prepared feathers and down and articles made of feathers or of down artificial flowers articles of human hair - Abrievated Graph Key: C285"@en-AU ;
    rdfs:subClassOf C2004A04997: ;
    skos:broader C2004A04997:286 ;
    skos:definition "Chapter 67 Prepared feathers and down and articles made of feathers or of down artificial flowers articles of human hair"@en-AU ;
    skos:narrower C2004A04997:277 ;
    skos:prefLabel "Chapter C285"@en-AU ;
    dcat:accessURL <https://www.legislation.gov.au/C2004A04997/2024-07-01/2024-07-01/text/1/epub/OEBPS/document_4/document_4.html#_Toc171752016> ;
    dcat:landingPage "https://www.legislation.gov.au/C2004A04997/2024-07-01/2024-07-01/text/1/epub/OEBPS/document_4/document_4.html#_Toc171752016"^^xsd:anyURI ;
    dcat:theme legcons:Chapter .

C2004A04997:288 a legcons:Chapter,
        C2004A04997:Chapter,
        owl:Class,
        dcat:Resource ;
    rdfs:label "Chapter - C288 Chapter 68 Articles of stone plaster cement asbestos mica or similar materials"@en-AU ;
    dct:hasPart C2004A04997:289 ;
    dct:isPartOf C2004A04997:287 ;
    rdfs:comment "Chapter 68 Articles of stone plaster cement asbestos mica or similar materials - Abrievated Graph Key: C288"@en-AU ;
    rdfs:subClassOf C2004A04997: ;
    skos:broader C2004A04997:289 ;
    skos:definition "Chapter 68 Articles of stone plaster cement asbestos mica or similar materials"@en-AU ;
    skos:narrower C2004A04997:287 ;
    skos:prefLabel "Chapter C288"@en-AU ;
    dcat:accessURL <https://www.legislation.gov.au/C2004A04997/2024-07-01/2024-07-01/text/1/epub/OEBPS/document_4/document_4.html#_Toc171752019> ;
    dcat:landingPage "https://www.legislation.gov.au/C2004A04997/2024-07-01/2024-07-01/text/1/epub/OEBPS/document_4/document_4.html#_Toc171752019"^^xsd:anyURI ;
    dcat:theme legcons:Chapter .

C2004A04997:297 a legcons:Section,
        C2004A04997:Section,
        owl:Class,
        dcat:Resource ;
    rdfs:label "Section - S297 Section XIVNatural or cultured pearls precious or semi precious stones precious metals metals clad with precious metal and articles thereof imitation jewellery coin"@en-AU ;
    dct:hasPart C2004A04997:298 ;
    dct:isPartOf C2004A04997:259 ;
    rdfs:comment "Section XIVNatural or cultured pearls precious or semi precious stones precious metals metals clad with precious metal and articles thereof imitation jewellery coin - Abrievated Graph Key: S297"@en-AU ;
    rdfs:subClassOf C2004A04997: ;
    skos:broader C2004A04997:298 ;
    skos:definition "Section XIVNatural or cultured pearls precious or semi precious stones precious metals metals clad with precious metal and articles thereof imitation jewellery coin"@en-AU ;
    skos:narrower C2004A04997:259 ;
    skos:prefLabel "Section S297"@en-AU ;
    dcat:accessURL <https://www.legislation.gov.au/C2004A04997/2024-07-01/2024-07-01/text/1/epub/OEBPS/document_4/document_4.html#_Toc171752028> ;
    dcat:landingPage "https://www.legislation.gov.au/C2004A04997/2024-07-01/2024-07-01/text/1/epub/OEBPS/document_4/document_4.html#_Toc171752028"^^xsd:anyURI ;
    dcat:theme legcons:Section .

C2004A04997:278 a legcons:Chapter,
        C2004A04997:Chapter,
        owl:Class,
        dcat:Resource ;
    rdfs:label "Chapter - C278 Chapter 64 Footwear gaiters and the like parts of such articles"@en-AU ;
    dct:hasPart C2004A04997:279,
        C2004A04997:280 ;
    dct:isPartOf C2004A04997:277 ;
    rdfs:comment "Chapter 64 Footwear gaiters and the like parts of such articles - Abrievated Graph Key: C278"@en-AU ;
    rdfs:subClassOf C2004A04997: ;
    skos:broader C2004A04997:279,
        C2004A04997:280 ;
    skos:definition "Chapter 64 Footwear gaiters and the like parts of such articles"@en-AU ;
    skos:narrower C2004A04997:277 ;
    skos:prefLabel "Chapter C278"@en-AU ;
    dcat:accessURL <https://www.legislation.gov.au/C2004A04997/2024-07-01/2024-07-01/text/1/epub/OEBPS/document_4/document_4.html#_Toc171752009> ;
    dcat:landingPage "https://www.legislation.gov.au/C2004A04997/2024-07-01/2024-07-01/text/1/epub/OEBPS/document_4/document_4.html#_Toc171752009"^^xsd:anyURI ;
    dcat:theme legcons:Chapter .

C2004A04997:294 a legcons:Chapter,
        C2004A04997:Chapter,
        owl:Class,
        dcat:Resource ;
    rdfs:label "Chapter - C294 Chapter 70 Glass and glassware"@en-AU ;
    dct:hasPart C2004A04997:295,
        C2004A04997:296 ;
    dct:isPartOf C2004A04997:287 ;
    rdfs:comment "Chapter 70 Glass and glassware - Abrievated Graph Key: C294"@en-AU ;
    rdfs:subClassOf C2004A04997: ;
    skos:broader C2004A04997:295,
        C2004A04997:296 ;
    skos:definition "Chapter 70 Glass and glassware"@en-AU ;
    skos:narrower C2004A04997:287 ;
    skos:prefLabel "Chapter C294"@en-AU ;
    dcat:accessURL <https://www.legislation.gov.au/C2004A04997/2024-07-01/2024-07-01/text/1/epub/OEBPS/document_4/document_4.html#_Toc171752025> ;
    dcat:landingPage "https://www.legislation.gov.au/C2004A04997/2024-07-01/2024-07-01/text/1/epub/OEBPS/document_4/document_4.html#_Toc171752025"^^xsd:anyURI ;
    dcat:theme legcons:Chapter .

C2004A04997:314 a legcons:Chapter,
        C2004A04997:Chapter,
        owl:Class,
        dcat:Resource ;
    rdfs:label "Chapter - C314 Chapter 73 Articles of iron or steel"@en-AU ;
    dct:hasPart C2004A04997:315,
        C2004A04997:316 ;
    dct:isPartOf C2004A04997:304 ;
    rdfs:comment "Chapter 73 Articles of iron or steel - Abrievated Graph Key: C314"@en-AU ;
    rdfs:subClassOf C2004A04997: ;
    skos:broader C2004A04997:315,
        C2004A04997:316 ;
    skos:definition "Chapter 73 Articles of iron or steel"@en-AU ;
    skos:narrower C2004A04997:304 ;
    skos:prefLabel "Chapter C314"@en-AU ;
    dcat:accessURL <https://www.legislation.gov.au/C2004A04997/2024-07-01/2024-07-01/text/1/epub/OEBPS/document_4/document_4.html#_Toc171752045> ;
    dcat:landingPage "https://www.legislation.gov.au/C2004A04997/2024-07-01/2024-07-01/text/1/epub/OEBPS/document_4/document_4.html#_Toc171752045"^^xsd:anyURI ;
    dcat:theme legcons:Chapter .

C2004A04997:287 a legcons:Section,
        C2004A04997:Section,
        owl:Class,
        dcat:Resource ;
    rdfs:label "Section - S287 Section XIIIArticles of stone plaster cement asbestos mica or similar materials ceramic products glass and glassware"@en-AU ;
    dct:hasPart C2004A04997:288,
        C2004A04997:290,
        C2004A04997:294 ;
    dct:isPartOf C2004A04997:259 ;
    rdfs:comment "Section XIIIArticles of stone plaster cement asbestos mica or similar materials ceramic products glass and glassware - Abrievated Graph Key: S287"@en-AU ;
    rdfs:subClassOf C2004A04997: ;
    skos:broader C2004A04997:288,
        C2004A04997:290,
        C2004A04997:294 ;
    skos:definition "Section XIIIArticles of stone plaster cement asbestos mica or similar materials ceramic products glass and glassware"@en-AU ;
    skos:narrower C2004A04997:259 ;
    skos:prefLabel "Section S287"@en-AU ;
    dcat:accessURL <https://www.legislation.gov.au/C2004A04997/2024-07-01/2024-07-01/text/1/epub/OEBPS/document_4/document_4.html#_Toc171752018> ;
    dcat:landingPage "https://www.legislation.gov.au/C2004A04997/2024-07-01/2024-07-01/text/1/epub/OEBPS/document_4/document_4.html#_Toc171752018"^^xsd:anyURI ;
    dcat:theme legcons:Section .

C2004A04997:290 a legcons:Chapter,
        C2004A04997:Chapter,
        owl:Class,
        dcat:Resource ;
    rdfs:label "Chapter - C290 Chapter 69 Ceramic products"@en-AU ;
    dct:hasPart C2004A04997:291,
        C2004A04997:292,
        C2004A04997:293 ;
    dct:isPartOf C2004A04997:287 ;
    rdfs:comment "Chapter 69 Ceramic products - Abrievated Graph Key: C290"@en-AU ;
    rdfs:subClassOf C2004A04997: ;
    skos:broader C2004A04997:291,
        C2004A04997:292,
        C2004A04997:293 ;
    skos:definition "Chapter 69 Ceramic products"@en-AU ;
    skos:narrower C2004A04997:287 ;
    skos:prefLabel "Chapter C290"@en-AU ;
    dcat:accessURL <https://www.legislation.gov.au/C2004A04997/2024-07-01/2024-07-01/text/1/epub/OEBPS/document_4/document_4.html#_Toc171752021> ;
    dcat:landingPage "https://www.legislation.gov.au/C2004A04997/2024-07-01/2024-07-01/text/1/epub/OEBPS/document_4/document_4.html#_Toc171752021"^^xsd:anyURI ;
    dcat:theme legcons:Chapter .

C2004A04997:304 a legcons:Section,
        C2004A04997:Section,
        owl:Class,
        dcat:Resource ;
    rdfs:label "Section - S304 Section XVBase metals and articles of base metal"@en-AU ;
    dct:hasPart C2004A04997:305,
        C2004A04997:306,
        C2004A04997:314 ;
    dct:isPartOf C2004A04997:259 ;
    rdfs:comment "Section XVBase metals and articles of base metal - Abrievated Graph Key: S304"@en-AU ;
    rdfs:subClassOf C2004A04997: ;
    skos:broader C2004A04997:305,
        C2004A04997:306,
        C2004A04997:314 ;
    skos:definition "Section XVBase metals and articles of base metal"@en-AU ;
    skos:narrower C2004A04997:259 ;
    skos:prefLabel "Section S304"@en-AU ;
    dcat:accessURL <https://www.legislation.gov.au/C2004A04997/2024-07-01/2024-07-01/text/1/epub/OEBPS/document_4/document_4.html#_Toc171752035> ;
    dcat:landingPage "https://www.legislation.gov.au/C2004A04997/2024-07-01/2024-07-01/text/1/epub/OEBPS/document_4/document_4.html#_Toc171752035"^^xsd:anyURI ;
    dcat:theme legcons:Section .

C2004A04997:56 a legcons:Part,
        C2004A04997:Part,
        owl:Class,
        dcat:Resource ;
    rdfs:label "Part - P56 Part 3 Miscellaneous"@en-AU ;
    dct:hasPart C2004A04997:57,
        C2004A04997:58,
        C2004A04997:59 ;
    dct:isPartOf C2004A04997:1 ;
    rdfs:comment "Part 3 Miscellaneous - Abrievated Graph Key: P56"@en-AU ;
    rdfs:subClassOf C2004A04997: ;
    skos:broader C2004A04997:57,
        C2004A04997:58,
        C2004A04997:59 ;
    skos:definition "Part 3 Miscellaneous"@en-AU ;
    skos:narrower C2004A04997:1 ;
    skos:prefLabel "Part P56"@en-AU ;
    dcat:accessURL <https://www.legislation.gov.au/C2004A04997/2024-07-01/2024-07-01/text/1/epub/OEBPS/document_1/document_1.html#_Toc172806556> ;
    dcat:landingPage "https://www.legislation.gov.au/C2004A04997/2024-07-01/2024-07-01/text/1/epub/OEBPS/document_1/document_1.html#_Toc172806556"^^xsd:anyURI ;
    dcat:theme legcons:Part .

C2004A04997:1 a legcons:Volume,
        C2004A04997:Volume,
        owl:Class,
        dcat:Resource ;
    rdfs:label "Volume - V1 Volume 1"@en-AU ;
    dct:hasPart C2004A04997:2,
        C2004A04997:36,
        C2004A04997:56,
        C2004A04997:60,
        C2004A04997:61 ;
    rdfs:comment "Volume 1 - Abrievated Graph Key: V1"@en-AU ;
    rdfs:subClassOf C2004A04997: ;
    skos:broader C2004A04997:2,
        C2004A04997:36,
        C2004A04997:56,
        C2004A04997:60,
        C2004A04997:61 ;
    skos:definition "Volume 1"@en-AU ;
    skos:prefLabel "Volume V1"@en-AU ;
    dcat:accessURL <https://www.legislation.gov.au/C2004A04997/2024-07-01/2024-07-01/text/1/epub/OEBPS/document_1/document_1.html> ;
    dcat:landingPage "https://www.legislation.gov.au/C2004A04997/2024-07-01/2024-07-01/text/1/epub/OEBPS/document_1/document_1.html"^^xsd:anyURI ;
    dcat:theme legcons:Volume .

C2004A04997:277 a legcons:Section,
        C2004A04997:Section,
        owl:Class,
        dcat:Resource ;
    rdfs:label "Section - S277 Section XIIFootwear headgear umbrellas sun umbrellas walking sticks seat sticks whips riding crops and parts thereof prepared feathers and articles made therewith artificial flowers articles of human hair"@en-AU ;
    dct:hasPart C2004A04997:278,
        C2004A04997:281,
        C2004A04997:283,
        C2004A04997:285 ;
    dct:isPartOf C2004A04997:259 ;
    rdfs:comment "Section XIIFootwear headgear umbrellas sun umbrellas walking sticks seat sticks whips riding crops and parts thereof prepared feathers and articles made therewith artificial flowers articles of human hair - Abrievated Graph Key: S277"@en-AU ;
    rdfs:subClassOf C2004A04997: ;
    skos:broader C2004A04997:278,
        C2004A04997:281,
        C2004A04997:283,
        C2004A04997:285 ;
    skos:definition "Section XIIFootwear headgear umbrellas sun umbrellas walking sticks seat sticks whips riding crops and parts thereof prepared feathers and articles made therewith artificial flowers articles of human hair"@en-AU ;
    skos:narrower C2004A04997:259 ;
    skos:prefLabel "Section S277"@en-AU ;
    dcat:accessURL <https://www.legislation.gov.au/C2004A04997/2024-07-01/2024-07-01/text/1/epub/OEBPS/document_4/document_4.html#_Toc171752008> ;
    dcat:landingPage "https://www.legislation.gov.au/C2004A04997/2024-07-01/2024-07-01/text/1/epub/OEBPS/document_4/document_4.html#_Toc171752008"^^xsd:anyURI ;
    dcat:theme legcons:Section .

C2004A04997:408 a legcons:Endnotes,
        C2004A04997:Endnotes,
        owl:Class,
        dcat:Resource ;
    rdfs:label "Endnotes - E408 Endnotes"@en-AU ;
    dct:hasPart C2004A04997:409,
        C2004A04997:410,
        C2004A04997:411,
        C2004A04997:412 ;
    dct:isPartOf C2004A04997:407 ;
    rdfs:comment "Endnotes - Abrievated Graph Key: E408"@en-AU ;
    rdfs:subClassOf C2004A04997: ;
    skos:broader C2004A04997:409,
        C2004A04997:410,
        C2004A04997:411,
        C2004A04997:412 ;
    skos:definition "Endnotes"@en-AU ;
    skos:narrower C2004A04997:407 ;
    skos:prefLabel "Endnotes E408"@en-AU ;
    dcat:accessURL <https://www.legislation.gov.au/C2004A04997/2024-07-01/2024-07-01/text/1/epub/OEBPS/document_7/document_7.html#_Toc171755738> ;
    dcat:landingPage "https://www.legislation.gov.au/C2004A04997/2024-07-01/2024-07-01/text/1/epub/OEBPS/document_7/document_7.html#_Toc171755738"^^xsd:anyURI ;
    dcat:theme legcons:Endnotes .

C2004A04997:259 a legcons:Volume,
        C2004A04997:Volume,
        owl:Class,
        dcat:Resource ;
    rdfs:label "Volume - V259 Volume 4"@en-AU ;
    dct:hasPart C2004A04997:260,
        C2004A04997:261,
        C2004A04997:277,
        C2004A04997:287,
        C2004A04997:297,
        C2004A04997:304 ;
    rdfs:comment "Volume 4 - Abrievated Graph Key: V259"@en-AU ;
    rdfs:subClassOf C2004A04997: ;
    skos:broader C2004A04997:260,
        C2004A04997:261,
        C2004A04997:277,
        C2004A04997:287,
        C2004A04997:297,
        C2004A04997:304 ;
    skos:definition "Volume 4"@en-AU ;
    skos:prefLabel "Volume V259"@en-AU ;
    dcat:accessURL <https://www.legislation.gov.au/C2004A04997/2024-07-01/2024-07-01/text/1/epub/OEBPS/document_4/document_4.html> ;
    dcat:landingPage "https://www.legislation.gov.au/C2004A04997/2024-07-01/2024-07-01/text/1/epub/OEBPS/document_4/document_4.html"^^xsd:anyURI ;
    dcat:theme legcons:Volume .

C2004A04997:298 a legcons:Chapter,
        C2004A04997:Chapter,
        owl:Class,
        dcat:Resource ;
    rdfs:label "Chapter - C298 Chapter 71 Natural or cultured pearls precious or semi precious stones precious metals metals clad with precious metal and articles thereof imitation jewellery coin"@en-AU ;
    dct:hasPart C2004A04997:299,
        C2004A04997:300,
        C2004A04997:301,
        C2004A04997:302,
        C2004A04997:303 ;
    dct:isPartOf C2004A04997:297 ;
    rdfs:comment "Chapter 71 Natural or cultured pearls precious or semi precious stones precious metals metals clad with precious metal and articles thereof imitation jewellery coin - Abrievated Graph Key: C298"@en-AU ;
    rdfs:subClassOf C2004A04997: ;
    skos:broader C2004A04997:299,
        C2004A04997:300,
        C2004A04997:301,
        C2004A04997:302,
        C2004A04997:303 ;
    skos:definition "Chapter 71 Natural or cultured pearls precious or semi precious stones precious metals metals clad with precious metal and articles thereof imitation jewellery coin"@en-AU ;
    skos:narrower C2004A04997:297 ;
    skos:prefLabel "Chapter C298"@en-AU ;
    dcat:accessURL <https://www.legislation.gov.au/C2004A04997/2024-07-01/2024-07-01/text/1/epub/OEBPS/document_4/document_4.html#_Toc171752029> ;
    dcat:landingPage "https://www.legislation.gov.au/C2004A04997/2024-07-01/2024-07-01/text/1/epub/OEBPS/document_4/document_4.html#_Toc171752029"^^xsd:anyURI ;
    dcat:theme legcons:Chapter .

C2004A04997:306 a legcons:Chapter,
        C2004A04997:Chapter,
        owl:Class,
        dcat:Resource ;
    rdfs:label "Chapter - C306 Chapter 72 Iron and steel"@en-AU ;
    dct:hasPart C2004A04997:307,
        C2004A04997:308,
        C2004A04997:309,
        C2004A04997:310,
        C2004A04997:311,
        C2004A04997:312,
        C2004A04997:313 ;
    dct:isPartOf C2004A04997:304 ;
    rdfs:comment "Chapter 72 Iron and steel - Abrievated Graph Key: C306"@en-AU ;
    rdfs:subClassOf C2004A04997: ;
    skos:broader C2004A04997:307,
        C2004A04997:308,
        C2004A04997:309,
        C2004A04997:310,
        C2004A04997:311,
        C2004A04997:312,
        C2004A04997:313 ;
    skos:definition "Chapter 72 Iron and steel"@en-AU ;
    skos:narrower C2004A04997:304 ;
    skos:prefLabel "Chapter C306"@en-AU ;
    dcat:accessURL <https://www.legislation.gov.au/C2004A04997/2024-07-01/2024-07-01/text/1/epub/OEBPS/document_4/document_4.html#_Toc171752037> ;
    dcat:landingPage "https://www.legislation.gov.au/C2004A04997/2024-07-01/2024-07-01/text/1/epub/OEBPS/document_4/document_4.html#_Toc171752037"^^xsd:anyURI ;
    dcat:theme legcons:Chapter .

C2004A04997:62 a legcons:Section,
        C2004A04997:Section,
        owl:Class,
        dcat:Resource ;
    rdfs:label "Section - S62 Section ILive animals animal products"@en-AU ;
    dct:hasPart C2004A04997:63,
        C2004A04997:64,
        C2004A04997:65,
        C2004A04997:66,
        C2004A04997:67,
        C2004A04997:68,
        C2004A04997:69,
        C2004A04997:70,
        C2004A04997:71,
        C2004A04997:72,
        C2004A04997:73,
        C2004A04997:74 ;
    dct:isPartOf C2004A04997:61 ;
    rdfs:comment "Section ILive animals animal products - Abrievated Graph Key: S62"@en-AU ;
    rdfs:subClassOf C2004A04997: ;
    skos:broader C2004A04997:63,
        C2004A04997:64,
        C2004A04997:65,
        C2004A04997:66,
        C2004A04997:67,
        C2004A04997:68,
        C2004A04997:69,
        C2004A04997:70,
        C2004A04997:71,
        C2004A04997:72,
        C2004A04997:73,
        C2004A04997:74 ;
    skos:definition "Section ILive animals animal products"@en-AU ;
    skos:narrower C2004A04997:61 ;
    skos:prefLabel "Section S62"@en-AU ;
    dcat:accessURL <https://www.legislation.gov.au/C2004A04997/2024-07-01/2024-07-01/text/1/epub/OEBPS/document_1/document_1.html#_Toc172806562> ;
    dcat:landingPage "https://www.legislation.gov.au/C2004A04997/2024-07-01/2024-07-01/text/1/epub/OEBPS/document_1/document_1.html#_Toc172806562"^^xsd:anyURI ;
    dcat:theme legcons:Section .

C2004A04997:261 a legcons:Section,
        C2004A04997:Section,
        owl:Class,
        dcat:Resource ;
    rdfs:label "Section - S261 Section XITextiles and textile articles"@en-AU ;
    dct:hasPart C2004A04997:262,
        C2004A04997:263,
        C2004A04997:264,
        C2004A04997:265,
        C2004A04997:266,
        C2004A04997:267,
        C2004A04997:268,
        C2004A04997:269,
        C2004A04997:270,
        C2004A04997:271,
        C2004A04997:272,
        C2004A04997:273,
        C2004A04997:274,
        C2004A04997:275,
        C2004A04997:276 ;
    dct:isPartOf C2004A04997:259 ;
    rdfs:comment "Section XITextiles and textile articles - Abrievated Graph Key: S261"@en-AU ;
    rdfs:subClassOf C2004A04997: ;
    skos:broader C2004A04997:262,
        C2004A04997:263,
        C2004A04997:264,
        C2004A04997:265,
        C2004A04997:266,
        C2004A04997:267,
        C2004A04997:268,
        C2004A04997:269,
        C2004A04997:270,
        C2004A04997:271,
        C2004A04997:272,
        C2004A04997:273,
        C2004A04997:274,
        C2004A04997:275,
        C2004A04997:276 ;
    skos:definition "Section XITextiles and textile articles"@en-AU ;
    skos:narrower C2004A04997:259 ;
    skos:prefLabel "Section S261"@en-AU ;
    dcat:accessURL <https://www.legislation.gov.au/C2004A04997/2024-07-01/2024-07-01/text/1/epub/OEBPS/document_4/document_4.html#_Toc171751992> ;
    dcat:landingPage "https://www.legislation.gov.au/C2004A04997/2024-07-01/2024-07-01/text/1/epub/OEBPS/document_4/document_4.html#_Toc171751992"^^xsd:anyURI ;
    dcat:theme legcons:Section .

C2004A04997:388 a legcons:Volume,
        C2004A04997:Volume,
        owl:Class,
        dcat:Resource ;
    rdfs:label "Volume - V388 Volume 6"@en-AU ;
    dct:hasPart C2004A04997:389,
        C2004A04997:390,
        C2004A04997:391,
        C2004A04997:392,
        C2004A04997:393,
        C2004A04997:394,
        C2004A04997:395,
        C2004A04997:396,
        C2004A04997:397,
        C2004A04997:398,
        C2004A04997:399,
        C2004A04997:400,
        C2004A04997:401,
        C2004A04997:402,
        C2004A04997:403,
        C2004A04997:404,
        C2004A04997:405,
        C2004A04997:406 ;
    rdfs:comment "Volume 6 - Abrievated Graph Key: V388"@en-AU ;
    rdfs:subClassOf C2004A04997: ;
    skos:broader C2004A04997:389,
        C2004A04997:390,
        C2004A04997:391,
        C2004A04997:392,
        C2004A04997:393,
        C2004A04997:394,
        C2004A04997:395,
        C2004A04997:396,
        C2004A04997:397,
        C2004A04997:398,
        C2004A04997:399,
        C2004A04997:400,
        C2004A04997:401,
        C2004A04997:402,
        C2004A04997:403,
        C2004A04997:404,
        C2004A04997:405,
        C2004A04997:406 ;
    skos:definition "Volume 6"@en-AU ;
    skos:prefLabel "Volume V388"@en-AU ;
    dcat:accessURL <https://www.legislation.gov.au/C2004A04997/2024-07-01/2024-07-01/text/1/epub/OEBPS/document_6/document_6.html> ;
    dcat:landingPage "https://www.legislation.gov.au/C2004A04997/2024-07-01/2024-07-01/text/1/epub/OEBPS/document_6/document_6.html"^^xsd:anyURI ;
    dcat:theme legcons:Volume .

C2004A04997:36 a legcons:Part,
        C2004A04997:Part,
        owl:Class,
        dcat:Resource ;
    rdfs:label "Part - P36 Part 2 Duties of Customs"@en-AU ;
    dct:hasPart C2004A04997:37,
        C2004A04997:38,
        C2004A04997:39,
        C2004A04997:40,
        C2004A04997:41,
        C2004A04997:42,
        C2004A04997:43,
        C2004A04997:44,
        C2004A04997:45,
        C2004A04997:46,
        C2004A04997:47,
        C2004A04997:48,
        C2004A04997:49,
        C2004A04997:50,
        C2004A04997:51,
        C2004A04997:52,
        C2004A04997:53,
        C2004A04997:54,
        C2004A04997:55 ;
    dct:isPartOf C2004A04997:1 ;
    rdfs:comment "Part 2 Duties of Customs - Abrievated Graph Key: P36"@en-AU ;
    rdfs:subClassOf C2004A04997: ;
    skos:broader C2004A04997:37,
        C2004A04997:38,
        C2004A04997:39,
        C2004A04997:40,
        C2004A04997:41,
        C2004A04997:42,
        C2004A04997:43,
        C2004A04997:44,
        C2004A04997:45,
        C2004A04997:46,
        C2004A04997:47,
        C2004A04997:48,
        C2004A04997:49,
        C2004A04997:50,
        C2004A04997:51,
        C2004A04997:52,
        C2004A04997:53,
        C2004A04997:54,
        C2004A04997:55 ;
    skos:definition "Part 2 Duties of Customs"@en-AU ;
    skos:narrower C2004A04997:1 ;
    skos:prefLabel "Part P36"@en-AU ;
    dcat:accessURL <https://www.legislation.gov.au/C2004A04997/2024-07-01/2024-07-01/text/1/epub/OEBPS/document_1/document_1.html#_Toc172806536> ;
    dcat:landingPage "https://www.legislation.gov.au/C2004A04997/2024-07-01/2024-07-01/text/1/epub/OEBPS/document_1/document_1.html#_Toc172806536"^^xsd:anyURI ;
    dcat:theme legcons:Part .

C2004A04997:61 a legcons:Schedule,
        C2004A04997:Schedule,
        owl:Class,
        dcat:Resource ;
    rdfs:label "Schedule - S61 Schedule 3 Classification of goods and general and special rates of duty"@en-AU ;
    dct:hasPart C2004A04997:100,
        C2004A04997:101,
        C2004A04997:62,
        C2004A04997:75,
        C2004A04997:76,
        C2004A04997:77,
        C2004A04997:78,
        C2004A04997:79,
        C2004A04997:80,
        C2004A04997:81,
        C2004A04997:82,
        C2004A04997:83,
        C2004A04997:84,
        C2004A04997:85,
        C2004A04997:86,
        C2004A04997:87,
        C2004A04997:88,
        C2004A04997:89,
        C2004A04997:90,
        C2004A04997:91,
        C2004A04997:92,
        C2004A04997:93,
        C2004A04997:94,
        C2004A04997:95,
        C2004A04997:96,
        C2004A04997:97,
        C2004A04997:98,
        C2004A04997:99 ;
    dct:isPartOf C2004A04997:1 ;
    rdfs:comment "Schedule 3 Classification of goods and general and special rates of duty - Abrievated Graph Key: S61"@en-AU ;
    rdfs:subClassOf C2004A04997: ;
    skos:broader C2004A04997:100,
        C2004A04997:101,
        C2004A04997:62,
        C2004A04997:75,
        C2004A04997:76,
        C2004A04997:77,
        C2004A04997:78,
        C2004A04997:79,
        C2004A04997:80,
        C2004A04997:81,
        C2004A04997:82,
        C2004A04997:83,
        C2004A04997:84,
        C2004A04997:85,
        C2004A04997:86,
        C2004A04997:87,
        C2004A04997:88,
        C2004A04997:89,
        C2004A04997:90,
        C2004A04997:91,
        C2004A04997:92,
        C2004A04997:93,
        C2004A04997:94,
        C2004A04997:95,
        C2004A04997:96,
        C2004A04997:97,
        C2004A04997:98,
        C2004A04997:99 ;
    skos:definition "Schedule 3 Classification of goods and general and special rates of duty"@en-AU ;
    skos:narrower C2004A04997:1 ;
    skos:prefLabel "Schedule S61"@en-AU ;
    dcat:accessURL <https://www.legislation.gov.au/C2004A04997/2024-07-01/2024-07-01/text/1/epub/OEBPS/document_1/document_1.html#_Toc172806561> ;
    dcat:landingPage "https://www.legislation.gov.au/C2004A04997/2024-07-01/2024-07-01/text/1/epub/OEBPS/document_1/document_1.html#_Toc172806561"^^xsd:anyURI ;
    dcat:theme legcons:Schedule .

C2004A04997:2 a legcons:Part,
        C2004A04997:Part,
        owl:Class,
        dcat:Resource ;
    rdfs:label "Part - P2 Part 1 Preliminary"@en-AU ;
    dct:hasPart C2004A04997:10,
        C2004A04997:11,
        C2004A04997:12,
        C2004A04997:13,
        C2004A04997:14,
        C2004A04997:15,
        C2004A04997:16,
        C2004A04997:17,
        C2004A04997:18,
        C2004A04997:19,
        C2004A04997:20,
        C2004A04997:21,
        C2004A04997:22,
        C2004A04997:23,
        C2004A04997:24,
        C2004A04997:25,
        C2004A04997:26,
        C2004A04997:27,
        C2004A04997:28,
        C2004A04997:29,
        C2004A04997:3,
        C2004A04997:30,
        C2004A04997:31,
        C2004A04997:32,
        C2004A04997:33,
        C2004A04997:34,
        C2004A04997:35,
        C2004A04997:4,
        C2004A04997:5,
        C2004A04997:6,
        C2004A04997:7,
        C2004A04997:8,
        C2004A04997:9 ;
    dct:isPartOf C2004A04997:1 ;
    rdfs:comment "Part 1 Preliminary - Abrievated Graph Key: P2"@en-AU ;
    rdfs:subClassOf C2004A04997: ;
    skos:broader C2004A04997:10,
        C2004A04997:11,
        C2004A04997:12,
        C2004A04997:13,
        C2004A04997:14,
        C2004A04997:15,
        C2004A04997:16,
        C2004A04997:17,
        C2004A04997:18,
        C2004A04997:19,
        C2004A04997:20,
        C2004A04997:21,
        C2004A04997:22,
        C2004A04997:23,
        C2004A04997:24,
        C2004A04997:25,
        C2004A04997:26,
        C2004A04997:27,
        C2004A04997:28,
        C2004A04997:29,
        C2004A04997:3,
        C2004A04997:30,
        C2004A04997:31,
        C2004A04997:32,
        C2004A04997:33,
        C2004A04997:34,
        C2004A04997:35,
        C2004A04997:4,
        C2004A04997:5,
        C2004A04997:6,
        C2004A04997:7,
        C2004A04997:8,
        C2004A04997:9 ;
    skos:definition "Part 1 Preliminary"@en-AU ;
    skos:narrower C2004A04997:1 ;
    skos:prefLabel "Part P2"@en-AU ;
    dcat:accessURL <https://www.legislation.gov.au/C2004A04997/2024-07-01/2024-07-01/text/1/epub/OEBPS/document_1/document_1.html#_Toc172806502> ;
    dcat:landingPage "https://www.legislation.gov.au/C2004A04997/2024-07-01/2024-07-01/text/1/epub/OEBPS/document_1/document_1.html#_Toc172806502"^^xsd:anyURI ;
    dcat:theme legcons:Part .

C2004A04997:198 a legcons:Schedule,
        C2004A04997:Schedule,
        owl:Class,
        dcat:Resource ;
    rdfs:label "Schedule - S198 Schedule 3 Classification of goods and general and special rates of duty"@en-AU ;
    dct:hasPart C2004A04997:199,
        C2004A04997:200,
        C2004A04997:201,
        C2004A04997:202,
        C2004A04997:203,
        C2004A04997:204,
        C2004A04997:205,
        C2004A04997:206,
        C2004A04997:207,
        C2004A04997:208,
        C2004A04997:209,
        C2004A04997:210,
        C2004A04997:211,
        C2004A04997:212,
        C2004A04997:213,
        C2004A04997:214,
        C2004A04997:215,
        C2004A04997:216,
        C2004A04997:217,
        C2004A04997:218,
        C2004A04997:219,
        C2004A04997:220,
        C2004A04997:221,
        C2004A04997:222,
        C2004A04997:223,
        C2004A04997:224,
        C2004A04997:225,
        C2004A04997:226,
        C2004A04997:227,
        C2004A04997:228,
        C2004A04997:229,
        C2004A04997:230,
        C2004A04997:231,
        C2004A04997:232,
        C2004A04997:233,
        C2004A04997:234,
        C2004A04997:235,
        C2004A04997:236,
        C2004A04997:237,
        C2004A04997:238,
        C2004A04997:239,
        C2004A04997:240,
        C2004A04997:241,
        C2004A04997:242,
        C2004A04997:243,
        C2004A04997:244,
        C2004A04997:245,
        C2004A04997:246,
        C2004A04997:247,
        C2004A04997:248,
        C2004A04997:249,
        C2004A04997:250,
        C2004A04997:251,
        C2004A04997:252,
        C2004A04997:253,
        C2004A04997:254,
        C2004A04997:255,
        C2004A04997:256,
        C2004A04997:257,
        C2004A04997:258 ;
    dct:isPartOf C2004A04997:197 ;
    rdfs:comment "Schedule 3 Classification of goods and general and special rates of duty - Abrievated Graph Key: S198"@en-AU ;
    rdfs:subClassOf C2004A04997: ;
    skos:broader C2004A04997:199,
        C2004A04997:200,
        C2004A04997:201,
        C2004A04997:202,
        C2004A04997:203,
        C2004A04997:204,
        C2004A04997:205,
        C2004A04997:206,
        C2004A04997:207,
        C2004A04997:208,
        C2004A04997:209,
        C2004A04997:210,
        C2004A04997:211,
        C2004A04997:212,
        C2004A04997:213,
        C2004A04997:214,
        C2004A04997:215,
        C2004A04997:216,
        C2004A04997:217,
        C2004A04997:218,
        C2004A04997:219,
        C2004A04997:220,
        C2004A04997:221,
        C2004A04997:222,
        C2004A04997:223,
        C2004A04997:224,
        C2004A04997:225,
        C2004A04997:226,
        C2004A04997:227,
        C2004A04997:228,
        C2004A04997:229,
        C2004A04997:230,
        C2004A04997:231,
        C2004A04997:232,
        C2004A04997:233,
        C2004A04997:234,
        C2004A04997:235,
        C2004A04997:236,
        C2004A04997:237,
        C2004A04997:238,
        C2004A04997:239,
        C2004A04997:240,
        C2004A04997:241,
        C2004A04997:242,
        C2004A04997:243,
        C2004A04997:244,
        C2004A04997:245,
        C2004A04997:246,
        C2004A04997:247,
        C2004A04997:248,
        C2004A04997:249,
        C2004A04997:250,
        C2004A04997:251,
        C2004A04997:252,
        C2004A04997:253,
        C2004A04997:254,
        C2004A04997:255,
        C2004A04997:256,
        C2004A04997:257,
        C2004A04997:258 ;
    skos:definition "Schedule 3 Classification of goods and general and special rates of duty"@en-AU ;
    skos:narrower C2004A04997:197 ;
    skos:prefLabel "Schedule S198"@en-AU ;
    dcat:accessURL <https://www.legislation.gov.au/C2004A04997/2024-07-01/2024-07-01/text/1/epub/OEBPS/document_3/document_3.html#_Toc171751528> ;
    dcat:landingPage "https://www.legislation.gov.au/C2004A04997/2024-07-01/2024-07-01/text/1/epub/OEBPS/document_3/document_3.html#_Toc171751528"^^xsd:anyURI ;
    dcat:theme legcons:Schedule .

C2004A04997:318 a legcons:Schedule,
        C2004A04997:Schedule,
        owl:Class,
        dcat:Resource ;
    rdfs:label "Schedule - S318 Schedule 3 Classification of goods and general and special rates of duty"@en-AU ;
    dct:hasPart C2004A04997:319,
        C2004A04997:320,
        C2004A04997:321,
        C2004A04997:322,
        C2004A04997:323,
        C2004A04997:324,
        C2004A04997:325,
        C2004A04997:326,
        C2004A04997:327,
        C2004A04997:328,
        C2004A04997:329,
        C2004A04997:330,
        C2004A04997:331,
        C2004A04997:332,
        C2004A04997:333,
        C2004A04997:334,
        C2004A04997:335,
        C2004A04997:336,
        C2004A04997:337,
        C2004A04997:338,
        C2004A04997:339,
        C2004A04997:340,
        C2004A04997:341,
        C2004A04997:342,
        C2004A04997:343,
        C2004A04997:344,
        C2004A04997:345,
        C2004A04997:346,
        C2004A04997:347,
        C2004A04997:348,
        C2004A04997:349,
        C2004A04997:350,
        C2004A04997:351,
        C2004A04997:352,
        C2004A04997:353,
        C2004A04997:354,
        C2004A04997:355,
        C2004A04997:356,
        C2004A04997:357,
        C2004A04997:358,
        C2004A04997:359,
        C2004A04997:360,
        C2004A04997:361,
        C2004A04997:362,
        C2004A04997:363,
        C2004A04997:364,
        C2004A04997:365,
        C2004A04997:366,
        C2004A04997:367,
        C2004A04997:368,
        C2004A04997:369,
        C2004A04997:370,
        C2004A04997:371,
        C2004A04997:372,
        C2004A04997:373,
        C2004A04997:374,
        C2004A04997:375,
        C2004A04997:376,
        C2004A04997:377,
        C2004A04997:378,
        C2004A04997:379,
        C2004A04997:380,
        C2004A04997:381,
        C2004A04997:382,
        C2004A04997:383,
        C2004A04997:384,
        C2004A04997:385,
        C2004A04997:386,
        C2004A04997:387 ;
    dct:isPartOf C2004A04997:317 ;
    rdfs:comment "Schedule 3 Classification of goods and general and special rates of duty - Abrievated Graph Key: S318"@en-AU ;
    rdfs:subClassOf C2004A04997: ;
    skos:broader C2004A04997:319,
        C2004A04997:320,
        C2004A04997:321,
        C2004A04997:322,
        C2004A04997:323,
        C2004A04997:324,
        C2004A04997:325,
        C2004A04997:326,
        C2004A04997:327,
        C2004A04997:328,
        C2004A04997:329,
        C2004A04997:330,
        C2004A04997:331,
        C2004A04997:332,
        C2004A04997:333,
        C2004A04997:334,
        C2004A04997:335,
        C2004A04997:336,
        C2004A04997:337,
        C2004A04997:338,
        C2004A04997:339,
        C2004A04997:340,
        C2004A04997:341,
        C2004A04997:342,
        C2004A04997:343,
        C2004A04997:344,
        C2004A04997:345,
        C2004A04997:346,
        C2004A04997:347,
        C2004A04997:348,
        C2004A04997:349,
        C2004A04997:350,
        C2004A04997:351,
        C2004A04997:352,
        C2004A04997:353,
        C2004A04997:354,
        C2004A04997:355,
        C2004A04997:356,
        C2004A04997:357,
        C2004A04997:358,
        C2004A04997:359,
        C2004A04997:360,
        C2004A04997:361,
        C2004A04997:362,
        C2004A04997:363,
        C2004A04997:364,
        C2004A04997:365,
        C2004A04997:366,
        C2004A04997:367,
        C2004A04997:368,
        C2004A04997:369,
        C2004A04997:370,
        C2004A04997:371,
        C2004A04997:372,
        C2004A04997:373,
        C2004A04997:374,
        C2004A04997:375,
        C2004A04997:376,
        C2004A04997:377,
        C2004A04997:378,
        C2004A04997:379,
        C2004A04997:380,
        C2004A04997:381,
        C2004A04997:382,
        C2004A04997:383,
        C2004A04997:384,
        C2004A04997:385,
        C2004A04997:386,
        C2004A04997:387 ;
    skos:definition "Schedule 3 Classification of goods and general and special rates of duty"@en-AU ;
    skos:narrower C2004A04997:317 ;
    skos:prefLabel "Schedule S318"@en-AU ;
    dcat:accessURL <https://www.legislation.gov.au/C2004A04997/2024-07-01/2024-07-01/text/1/epub/OEBPS/document_5/document_5.html#_Toc171753160> ;
    dcat:landingPage "https://www.legislation.gov.au/C2004A04997/2024-07-01/2024-07-01/text/1/epub/OEBPS/document_5/document_5.html#_Toc171753160"^^xsd:anyURI ;
    dcat:theme legcons:Schedule .

C2004A04997:103 a legcons:Schedule,
        C2004A04997:Schedule,
        owl:Class,
        dcat:Resource ;
    rdfs:label "Schedule - S103 Schedule 3 Classification of goods and general and special rates of duty"@en-AU ;
    dct:hasPart C2004A04997:104,
        C2004A04997:105,
        C2004A04997:106,
        C2004A04997:107,
        C2004A04997:108,
        C2004A04997:109,
        C2004A04997:110,
        C2004A04997:111,
        C2004A04997:112,
        C2004A04997:113,
        C2004A04997:114,
        C2004A04997:115,
        C2004A04997:116,
        C2004A04997:117,
        C2004A04997:118,
        C2004A04997:119,
        C2004A04997:120,
        C2004A04997:121,
        C2004A04997:122,
        C2004A04997:123,
        C2004A04997:124,
        C2004A04997:125,
        C2004A04997:126,
        C2004A04997:127,
        C2004A04997:128,
        C2004A04997:129,
        C2004A04997:130,
        C2004A04997:131,
        C2004A04997:132,
        C2004A04997:133,
        C2004A04997:134,
        C2004A04997:135,
        C2004A04997:136,
        C2004A04997:137,
        C2004A04997:138,
        C2004A04997:139,
        C2004A04997:140,
        C2004A04997:141,
        C2004A04997:142,
        C2004A04997:143,
        C2004A04997:144,
        C2004A04997:145,
        C2004A04997:146,
        C2004A04997:147,
        C2004A04997:148,
        C2004A04997:149,
        C2004A04997:150,
        C2004A04997:151,
        C2004A04997:152,
        C2004A04997:153,
        C2004A04997:154,
        C2004A04997:155,
        C2004A04997:156,
        C2004A04997:157,
        C2004A04997:158,
        C2004A04997:159,
        C2004A04997:160,
        C2004A04997:161,
        C2004A04997:162,
        C2004A04997:163,
        C2004A04997:164,
        C2004A04997:165,
        C2004A04997:166,
        C2004A04997:167,
        C2004A04997:168,
        C2004A04997:169,
        C2004A04997:170,
        C2004A04997:171,
        C2004A04997:172,
        C2004A04997:173,
        C2004A04997:174,
        C2004A04997:175,
        C2004A04997:176,
        C2004A04997:177,
        C2004A04997:178,
        C2004A04997:179,
        C2004A04997:180,
        C2004A04997:181,
        C2004A04997:182,
        C2004A04997:183,
        C2004A04997:184,
        C2004A04997:185,
        C2004A04997:186,
        C2004A04997:187,
        C2004A04997:188,
        C2004A04997:189,
        C2004A04997:190,
        C2004A04997:191,
        C2004A04997:192,
        C2004A04997:193,
        C2004A04997:194,
        C2004A04997:195,
        C2004A04997:196 ;
    dct:isPartOf C2004A04997:102 ;
    rdfs:comment "Schedule 3 Classification of goods and general and special rates of duty - Abrievated Graph Key: S103"@en-AU ;
    rdfs:subClassOf C2004A04997: ;
    skos:broader C2004A04997:104,
        C2004A04997:105,
        C2004A04997:106,
        C2004A04997:107,
        C2004A04997:108,
        C2004A04997:109,
        C2004A04997:110,
        C2004A04997:111,
        C2004A04997:112,
        C2004A04997:113,
        C2004A04997:114,
        C2004A04997:115,
        C2004A04997:116,
        C2004A04997:117,
        C2004A04997:118,
        C2004A04997:119,
        C2004A04997:120,
        C2004A04997:121,
        C2004A04997:122,
        C2004A04997:123,
        C2004A04997:124,
        C2004A04997:125,
        C2004A04997:126,
        C2004A04997:127,
        C2004A04997:128,
        C2004A04997:129,
        C2004A04997:130,
        C2004A04997:131,
        C2004A04997:132,
        C2004A04997:133,
        C2004A04997:134,
        C2004A04997:135,
        C2004A04997:136,
        C2004A04997:137,
        C2004A04997:138,
        C2004A04997:139,
        C2004A04997:140,
        C2004A04997:141,
        C2004A04997:142,
        C2004A04997:143,
        C2004A04997:144,
        C2004A04997:145,
        C2004A04997:146,
        C2004A04997:147,
        C2004A04997:148,
        C2004A04997:149,
        C2004A04997:150,
        C2004A04997:151,
        C2004A04997:152,
        C2004A04997:153,
        C2004A04997:154,
        C2004A04997:155,
        C2004A04997:156,
        C2004A04997:157,
        C2004A04997:158,
        C2004A04997:159,
        C2004A04997:160,
        C2004A04997:161,
        C2004A04997:162,
        C2004A04997:163,
        C2004A04997:164,
        C2004A04997:165,
        C2004A04997:166,
        C2004A04997:167,
        C2004A04997:168,
        C2004A04997:169,
        C2004A04997:170,
        C2004A04997:171,
        C2004A04997:172,
        C2004A04997:173,
        C2004A04997:174,
        C2004A04997:175,
        C2004A04997:176,
        C2004A04997:177,
        C2004A04997:178,
        C2004A04997:179,
        C2004A04997:180,
        C2004A04997:181,
        C2004A04997:182,
        C2004A04997:183,
        C2004A04997:184,
        C2004A04997:185,
        C2004A04997:186,
        C2004A04997:187,
        C2004A04997:188,
        C2004A04997:189,
        C2004A04997:190,
        C2004A04997:191,
        C2004A04997:192,
        C2004A04997:193,
        C2004A04997:194,
        C2004A04997:195,
        C2004A04997:196 ;
    skos:definition "Schedule 3 Classification of goods and general and special rates of duty"@en-AU ;
    skos:narrower C2004A04997:102 ;
    skos:prefLabel "Schedule S103"@en-AU ;
    dcat:accessURL <https://www.legislation.gov.au/C2004A04997/2024-07-01/2024-07-01/text/1/epub/OEBPS/document_2/document_2.html#_Toc171750929> ;
    dcat:landingPage "https://www.legislation.gov.au/C2004A04997/2024-07-01/2024-07-01/text/1/epub/OEBPS/document_2/document_2.html#_Toc171750929"^^xsd:anyURI ;
    dcat:theme legcons:Schedule .

C2004A04997: a owl:Class,
        dcat:Dataset,
        dcat:Resource ;
    rdfs:label "Customs Tariff Act 1995" ;
    dct:Agent "Home Affairs"@en-AU ;
    dct:created "2024-08-21T09:11:49.666522"^^xsd:dateTime ;
    dct:creator "https://orcid.org/0009-0007-8434-7325"^^xsd:anyURI ;
    dct:date "2024-07-01T00:00:00+10:00"^^xsd:dateTime ;
    dct:description "Customs Tariff Act 1995"@en-AU ;
    dct:identifier "https://www.legislation.gov.au/C2004A04997/latest"^^xsd:anyURI ;
    dct:license <https://creativecommons.org/licenses/by-sa/4.0/> ;
    dct:publisher "Department of Home Affairs" ;
    dct:source "scheme=AGLSTERMS.AglsAgent; corporateName=Office Parliamentary Counsel; address=Locked Bag 30 Kingston ACT 2604; contact=+61 2 6120 1400"@en-AU ;
    dct:subject "Customs Tariff Act 1995"@en-AU ;
    dct:title "Customs Tariff Act 1995"@en-AU ;
    owl:imports legcons: ;
    dcat:theme legcons:Chapter,
        legcons:Endnotes,
        legcons:Item,
        legcons:Part,
        legcons:Schedule,
        legcons:Section,
        legcons:Volume ;
    schema:identifier "C2004A04997" ;
    schema:status "In force" ;
    schema:version "C2024C00273 (C92)" .

