@prefix C2004A04997: <http://example.org/au/leg/dataset/C2004A04997/> .
@prefix dcat: <http://www.w3.org/ns/dcat#> .
@prefix dt: <http://purl.org/dc/terms/> .
@prefix legcons: <http://example.org/au/leg/concepts/> .
@prefix owl: <http://www.w3.org/2002/07/owl#> .
@prefix rdfs: <http://www.w3.org/2000/01/rdf-schema#> .
@prefix schema: <https://schema.org/> .
@prefix skos: <http://www.w3.org/2004/02/skos/core#> .
@prefix xsd: <http://www.w3.org/2001/XMLSchema#> .

C2004A04997: a owl:Ontology,
        dcat:Dataset ;
    dt:Agent "Home Affairs"@en-AU ;
    dt:created "2024-08-05T21:38:51.013312"^^xsd:dateTime ;
    dt:creator "https://orcid.org/0009-0007-8434-7325"^^xsd:anyURI ;
    dt:date "2024-07-01T00:00:00+10:00"^^xsd:dateTime ;
    dt:description "Customs Tariff Act 1995"@en-AU ;
    dt:identifier "https://www.legislation.gov.au/C2004A04997/latest"^^xsd:anyURI ;
    dt:publisher "Department of Home Affairs" ;
    dt:source "scheme=AGLSTERMS.AglsAgent; corporateName=Office Parliamentary Counsel; address=Locked Bag 30 Kingston ACT 2604; contact=+61 2 6120 1400"@en-AU ;
    dt:subject "Customs Tariff Act 1995"@en-AU ;
    dt:title "Customs Tariff Act 1995"@en-AU ;
    owl:imports legcons: ;
    schema:identifier "C2004A04997" ;
    schema:status "In force" ;
    schema:version "C2024C00273 (C92)" .

C2004A04997:388 a legcons:Volume,
        skos:Concept,
        dcat:Resource ;
    rdfs:label "Volume V388"@en-AU ;
    rdfs:comment "Volume 6 - GraphNodeID: V388"@en-AU ;
    skos:definition "Volume 6"@en-AU ;
    skos:prefLabel "Volume V388"@en-AU ;
    dcat:accessURL "https://www.legislation.gov.au/C2004A04997/2024-07-01/2024-07-01/text/1/epub/OEBPS/document_6/document_6.html"^^xsd:anyURI .

C2004A04997:407 a legcons:Volume,
        skos:Concept,
        dcat:Resource ;
    rdfs:label "Volume V407"@en-AU ;
    rdfs:comment "Volume 7 - GraphNodeID: V407"@en-AU ;
    skos:definition "Volume 7"@en-AU ;
    skos:prefLabel "Volume V407"@en-AU ;
    dcat:accessURL "https://www.legislation.gov.au/C2004A04997/2024-07-01/2024-07-01/text/1/epub/OEBPS/document_7/document_7.html"^^xsd:anyURI .

C2004A04997:10 a legcons:Item,
        skos:Concept,
        dcat:Resource ;
    rdfs:label "Item I10"@en-AU ;
    rdfs:comment "7  Rules for classifying goods in Schedule 3 - GraphNodeID: I10"@en-AU ;
    skos:definition "7  Rules for classifying goods in Schedule 3"@en-AU ;
    skos:narrower C2004A04997:2 ;
    skos:prefLabel "Item I10"@en-AU ;
    dcat:accessURL "https://www.legislation.gov.au/C2004A04997/2024-07-01/2024-07-01/text/1/epub/OEBPS/document_1/document_1.html#_Toc172806510"^^xsd:anyURI .

C2004A04997:100 a legcons:Item,
        skos:Concept,
        dcat:Resource ;
    rdfs:label "Item I100"@en-AU ;
    rdfs:comment "Subheading Notes - GraphNodeID: I100"@en-AU ;
    skos:definition "Subheading Notes"@en-AU ;
    skos:narrower C2004A04997:56 ;
    skos:prefLabel "Item I100"@en-AU ;
    dcat:accessURL "https://www.legislation.gov.au/C2004A04997/2024-07-01/2024-07-01/text/1/epub/OEBPS/document_1/document_1.html#_Toc172806600"^^xsd:anyURI .

C2004A04997:101 a legcons:Item,
        skos:Concept,
        dcat:Resource ;
    rdfs:label "Item I101"@en-AU ;
    rdfs:comment "Additional Note - GraphNodeID: I101"@en-AU ;
    skos:definition "Additional Note"@en-AU ;
    skos:narrower C2004A04997:56 ;
    skos:prefLabel "Item I101"@en-AU ;
    dcat:accessURL "https://www.legislation.gov.au/C2004A04997/2024-07-01/2024-07-01/text/1/epub/OEBPS/document_1/document_1.html#_Toc172806601"^^xsd:anyURI .

C2004A04997:103 a legcons:Item,
        skos:Concept,
        dcat:Resource ;
    rdfs:label "Item I103"@en-AU ;
    rdfs:comment "Schedule 3 Classification of goods and general and special rates of duty - GraphNodeID: I103"@en-AU ;
    skos:definition "Schedule 3 Classification of goods and general and special rates of duty"@en-AU ;
    skos:narrower C2004A04997:56 ;
    skos:prefLabel "Item I103"@en-AU ;
    dcat:accessURL "https://www.legislation.gov.au/C2004A04997/2024-07-01/2024-07-01/text/1/epub/OEBPS/document_2/document_2.html#_Toc171750929"^^xsd:anyURI .

C2004A04997:104 a legcons:Item,
        skos:Concept,
        dcat:Resource ;
    rdfs:label "Item I104"@en-AU ;
    rdfs:comment "Section IVPrepared foodstuffs beverages spirits and vinegar tobacco and manufactured tobacco substitutes products whether or not containing nicotine intended for inhalation without combustion other nicotine containing products intended for the intake of nicotine into the human body - GraphNodeID: I104"@en-AU ;
    skos:definition "Section IVPrepared foodstuffs beverages spirits and vinegar tobacco and manufactured tobacco substitutes products whether or not containing nicotine intended for inhalation without combustion other nicotine containing products intended for the intake of nicotine into the human body"@en-AU ;
    skos:narrower C2004A04997:56 ;
    skos:prefLabel "Item I104"@en-AU ;
    dcat:accessURL "https://www.legislation.gov.au/C2004A04997/2024-07-01/2024-07-01/text/1/epub/OEBPS/document_2/document_2.html#_Toc171750930"^^xsd:anyURI .

C2004A04997:105 a legcons:Item,
        skos:Concept,
        dcat:Resource ;
    rdfs:label "Item I105"@en-AU ;
    rdfs:comment "Note - GraphNodeID: I105"@en-AU ;
    skos:definition "Note"@en-AU ;
    skos:narrower C2004A04997:56 ;
    skos:prefLabel "Item I105"@en-AU ;
    dcat:accessURL "https://www.legislation.gov.au/C2004A04997/2024-07-01/2024-07-01/text/1/epub/OEBPS/document_2/document_2.html#_Toc171750931"^^xsd:anyURI .

C2004A04997:106 a legcons:Item,
        skos:Concept,
        dcat:Resource ;
    rdfs:label "Item I106"@en-AU ;
    rdfs:comment "Additional Note - GraphNodeID: I106"@en-AU ;
    skos:definition "Additional Note"@en-AU ;
    skos:narrower C2004A04997:56 ;
    skos:prefLabel "Item I106"@en-AU ;
    dcat:accessURL "https://www.legislation.gov.au/C2004A04997/2024-07-01/2024-07-01/text/1/epub/OEBPS/document_2/document_2.html#_Toc171750932"^^xsd:anyURI .

C2004A04997:107 a legcons:Chapter,
        skos:Concept,
        dcat:Resource ;
    rdfs:label "Chapter C107"@en-AU ;
    rdfs:comment "Chapter 16 Preparations of meat of fish of crustaceans molluscs or other aquatic invertebrates or of insects - GraphNodeID: C107"@en-AU ;
    skos:definition "Chapter 16 Preparations of meat of fish of crustaceans molluscs or other aquatic invertebrates or of insects"@en-AU ;
    skos:narrower C2004A04997:102 ;
    skos:prefLabel "Chapter C107"@en-AU ;
    dcat:accessURL "https://www.legislation.gov.au/C2004A04997/2024-07-01/2024-07-01/text/1/epub/OEBPS/document_2/document_2.html#_Toc171750933"^^xsd:anyURI .

C2004A04997:108 a legcons:Item,
        skos:Concept,
        dcat:Resource ;
    rdfs:label "Item I108"@en-AU ;
    rdfs:comment "Notes - GraphNodeID: I108"@en-AU ;
    skos:definition "Notes"@en-AU ;
    skos:narrower C2004A04997:56 ;
    skos:prefLabel "Item I108"@en-AU ;
    dcat:accessURL "https://www.legislation.gov.au/C2004A04997/2024-07-01/2024-07-01/text/1/epub/OEBPS/document_2/document_2.html#_Toc171750934"^^xsd:anyURI .

C2004A04997:109 a legcons:Item,
        skos:Concept,
        dcat:Resource ;
    rdfs:label "Item I109"@en-AU ;
    rdfs:comment "Subheading Notes - GraphNodeID: I109"@en-AU ;
    skos:definition "Subheading Notes"@en-AU ;
    skos:narrower C2004A04997:56 ;
    skos:prefLabel "Item I109"@en-AU ;
    dcat:accessURL "https://www.legislation.gov.au/C2004A04997/2024-07-01/2024-07-01/text/1/epub/OEBPS/document_2/document_2.html#_Toc171750935"^^xsd:anyURI .

C2004A04997:11 a legcons:Item,
        skos:Concept,
        dcat:Resource ;
    rdfs:label "Item I11"@en-AU ;
    rdfs:comment "8  Application of Schedule 4 - GraphNodeID: I11"@en-AU ;
    skos:definition "8  Application of Schedule 4"@en-AU ;
    skos:narrower C2004A04997:2 ;
    skos:prefLabel "Item I11"@en-AU ;
    dcat:accessURL "https://www.legislation.gov.au/C2004A04997/2024-07-01/2024-07-01/text/1/epub/OEBPS/document_1/document_1.html#_Toc172806511"^^xsd:anyURI .

C2004A04997:110 a legcons:Chapter,
        skos:Concept,
        dcat:Resource ;
    rdfs:label "Chapter C110"@en-AU ;
    rdfs:comment "Chapter 17 Sugars and sugar confectionery - GraphNodeID: C110"@en-AU ;
    skos:definition "Chapter 17 Sugars and sugar confectionery"@en-AU ;
    skos:narrower C2004A04997:102 ;
    skos:prefLabel "Chapter C110"@en-AU ;
    dcat:accessURL "https://www.legislation.gov.au/C2004A04997/2024-07-01/2024-07-01/text/1/epub/OEBPS/document_2/document_2.html#_Toc171750936"^^xsd:anyURI .

C2004A04997:111 a legcons:Item,
        skos:Concept,
        dcat:Resource ;
    rdfs:label "Item I111"@en-AU ;
    rdfs:comment "Note - GraphNodeID: I111"@en-AU ;
    skos:definition "Note"@en-AU ;
    skos:narrower C2004A04997:56 ;
    skos:prefLabel "Item I111"@en-AU ;
    dcat:accessURL "https://www.legislation.gov.au/C2004A04997/2024-07-01/2024-07-01/text/1/epub/OEBPS/document_2/document_2.html#_Toc171750937"^^xsd:anyURI .

C2004A04997:112 a legcons:Item,
        skos:Concept,
        dcat:Resource ;
    rdfs:label "Item I112"@en-AU ;
    rdfs:comment "Subheading Notes - GraphNodeID: I112"@en-AU ;
    skos:definition "Subheading Notes"@en-AU ;
    skos:narrower C2004A04997:56 ;
    skos:prefLabel "Item I112"@en-AU ;
    dcat:accessURL "https://www.legislation.gov.au/C2004A04997/2024-07-01/2024-07-01/text/1/epub/OEBPS/document_2/document_2.html#_Toc171750938"^^xsd:anyURI .

C2004A04997:113 a legcons:Chapter,
        skos:Concept,
        dcat:Resource ;
    rdfs:label "Chapter C113"@en-AU ;
    rdfs:comment "Chapter 18 Cocoa and cocoa preparations - GraphNodeID: C113"@en-AU ;
    skos:definition "Chapter 18 Cocoa and cocoa preparations"@en-AU ;
    skos:narrower C2004A04997:102 ;
    skos:prefLabel "Chapter C113"@en-AU ;
    dcat:accessURL "https://www.legislation.gov.au/C2004A04997/2024-07-01/2024-07-01/text/1/epub/OEBPS/document_2/document_2.html#_Toc171750939"^^xsd:anyURI .

C2004A04997:114 a legcons:Item,
        skos:Concept,
        dcat:Resource ;
    rdfs:label "Item I114"@en-AU ;
    rdfs:comment "Notes - GraphNodeID: I114"@en-AU ;
    skos:definition "Notes"@en-AU ;
    skos:narrower C2004A04997:56 ;
    skos:prefLabel "Item I114"@en-AU ;
    dcat:accessURL "https://www.legislation.gov.au/C2004A04997/2024-07-01/2024-07-01/text/1/epub/OEBPS/document_2/document_2.html#_Toc171750940"^^xsd:anyURI .

C2004A04997:115 a legcons:Chapter,
        skos:Concept,
        dcat:Resource ;
    rdfs:label "Chapter C115"@en-AU ;
    rdfs:comment "Chapter 19 Preparations of cereals flour starch or milk pastrycooks products - GraphNodeID: C115"@en-AU ;
    skos:definition "Chapter 19 Preparations of cereals flour starch or milk pastrycooks products"@en-AU ;
    skos:narrower C2004A04997:102 ;
    skos:prefLabel "Chapter C115"@en-AU ;
    dcat:accessURL "https://www.legislation.gov.au/C2004A04997/2024-07-01/2024-07-01/text/1/epub/OEBPS/document_2/document_2.html#_Toc171750941"^^xsd:anyURI .

C2004A04997:116 a legcons:Item,
        skos:Concept,
        dcat:Resource ;
    rdfs:label "Item I116"@en-AU ;
    rdfs:comment "Notes - GraphNodeID: I116"@en-AU ;
    skos:definition "Notes"@en-AU ;
    skos:narrower C2004A04997:56 ;
    skos:prefLabel "Item I116"@en-AU ;
    dcat:accessURL "https://www.legislation.gov.au/C2004A04997/2024-07-01/2024-07-01/text/1/epub/OEBPS/document_2/document_2.html#_Toc171750942"^^xsd:anyURI .

C2004A04997:117 a legcons:Item,
        skos:Concept,
        dcat:Resource ;
    rdfs:label "Item I117"@en-AU ;
    rdfs:comment "Additional Note - GraphNodeID: I117"@en-AU ;
    skos:definition "Additional Note"@en-AU ;
    skos:narrower C2004A04997:56 ;
    skos:prefLabel "Item I117"@en-AU ;
    dcat:accessURL "https://www.legislation.gov.au/C2004A04997/2024-07-01/2024-07-01/text/1/epub/OEBPS/document_2/document_2.html#_Toc171750943"^^xsd:anyURI .

C2004A04997:118 a legcons:Chapter,
        skos:Concept,
        dcat:Resource ;
    rdfs:label "Chapter C118"@en-AU ;
    rdfs:comment "Chapter 20 Preparations of vegetables fruit nuts or other parts of plants - GraphNodeID: C118"@en-AU ;
    skos:definition "Chapter 20 Preparations of vegetables fruit nuts or other parts of plants"@en-AU ;
    skos:narrower C2004A04997:102 ;
    skos:prefLabel "Chapter C118"@en-AU ;
    dcat:accessURL "https://www.legislation.gov.au/C2004A04997/2024-07-01/2024-07-01/text/1/epub/OEBPS/document_2/document_2.html#_Toc171750944"^^xsd:anyURI .

C2004A04997:119 a legcons:Item,
        skos:Concept,
        dcat:Resource ;
    rdfs:label "Item I119"@en-AU ;
    rdfs:comment "Notes - GraphNodeID: I119"@en-AU ;
    skos:definition "Notes"@en-AU ;
    skos:narrower C2004A04997:56 ;
    skos:prefLabel "Item I119"@en-AU ;
    dcat:accessURL "https://www.legislation.gov.au/C2004A04997/2024-07-01/2024-07-01/text/1/epub/OEBPS/document_2/document_2.html#_Toc171750945"^^xsd:anyURI .

C2004A04997:12 a legcons:Item,
        skos:Concept,
        dcat:Resource ;
    rdfs:label "Item I12"@en-AU ;
    rdfs:comment "9  Rates of dutyad valorem duties - GraphNodeID: I12"@en-AU ;
    skos:definition "9  Rates of dutyad valorem duties"@en-AU ;
    skos:narrower C2004A04997:2 ;
    skos:prefLabel "Item I12"@en-AU ;
    dcat:accessURL "https://www.legislation.gov.au/C2004A04997/2024-07-01/2024-07-01/text/1/epub/OEBPS/document_1/document_1.html#_Toc172806512"^^xsd:anyURI .

C2004A04997:120 a legcons:Item,
        skos:Concept,
        dcat:Resource ;
    rdfs:label "Item I120"@en-AU ;
    rdfs:comment "Subheading Notes - GraphNodeID: I120"@en-AU ;
    skos:definition "Subheading Notes"@en-AU ;
    skos:narrower C2004A04997:56 ;
    skos:prefLabel "Item I120"@en-AU ;
    dcat:accessURL "https://www.legislation.gov.au/C2004A04997/2024-07-01/2024-07-01/text/1/epub/OEBPS/document_2/document_2.html#_Toc171750946"^^xsd:anyURI .

C2004A04997:121 a legcons:Item,
        skos:Concept,
        dcat:Resource ;
    rdfs:label "Item I121"@en-AU ;
    rdfs:comment "Additional Notes - GraphNodeID: I121"@en-AU ;
    skos:definition "Additional Notes"@en-AU ;
    skos:narrower C2004A04997:56 ;
    skos:prefLabel "Item I121"@en-AU ;
    dcat:accessURL "https://www.legislation.gov.au/C2004A04997/2024-07-01/2024-07-01/text/1/epub/OEBPS/document_2/document_2.html#_Toc171750947"^^xsd:anyURI .

C2004A04997:122 a legcons:Chapter,
        skos:Concept,
        dcat:Resource ;
    rdfs:label "Chapter C122"@en-AU ;
    rdfs:comment "Chapter 21 Miscellaneous edible preparations - GraphNodeID: C122"@en-AU ;
    skos:definition "Chapter 21 Miscellaneous edible preparations"@en-AU ;
    skos:narrower C2004A04997:102 ;
    skos:prefLabel "Chapter C122"@en-AU ;
    dcat:accessURL "https://www.legislation.gov.au/C2004A04997/2024-07-01/2024-07-01/text/1/epub/OEBPS/document_2/document_2.html#_Toc171750948"^^xsd:anyURI .

C2004A04997:123 a legcons:Item,
        skos:Concept,
        dcat:Resource ;
    rdfs:label "Item I123"@en-AU ;
    rdfs:comment "Notes - GraphNodeID: I123"@en-AU ;
    skos:definition "Notes"@en-AU ;
    skos:narrower C2004A04997:56 ;
    skos:prefLabel "Item I123"@en-AU ;
    dcat:accessURL "https://www.legislation.gov.au/C2004A04997/2024-07-01/2024-07-01/text/1/epub/OEBPS/document_2/document_2.html#_Toc171750949"^^xsd:anyURI .

C2004A04997:124 a legcons:Item,
        skos:Concept,
        dcat:Resource ;
    rdfs:label "Item I124"@en-AU ;
    rdfs:comment "Additional Notes - GraphNodeID: I124"@en-AU ;
    skos:definition "Additional Notes"@en-AU ;
    skos:narrower C2004A04997:56 ;
    skos:prefLabel "Item I124"@en-AU ;
    dcat:accessURL "https://www.legislation.gov.au/C2004A04997/2024-07-01/2024-07-01/text/1/epub/OEBPS/document_2/document_2.html#_Toc171750950"^^xsd:anyURI .

C2004A04997:125 a legcons:Chapter,
        skos:Concept,
        dcat:Resource ;
    rdfs:label "Chapter C125"@en-AU ;
    rdfs:comment "Chapter 22 Beverages spirits and vinegar - GraphNodeID: C125"@en-AU ;
    skos:definition "Chapter 22 Beverages spirits and vinegar"@en-AU ;
    skos:narrower C2004A04997:102 ;
    skos:prefLabel "Chapter C125"@en-AU ;
    dcat:accessURL "https://www.legislation.gov.au/C2004A04997/2024-07-01/2024-07-01/text/1/epub/OEBPS/document_2/document_2.html#_Toc171750951"^^xsd:anyURI .

C2004A04997:126 a legcons:Item,
        skos:Concept,
        dcat:Resource ;
    rdfs:label "Item I126"@en-AU ;
    rdfs:comment "Notes - GraphNodeID: I126"@en-AU ;
    skos:definition "Notes"@en-AU ;
    skos:narrower C2004A04997:56 ;
    skos:prefLabel "Item I126"@en-AU ;
    dcat:accessURL "https://www.legislation.gov.au/C2004A04997/2024-07-01/2024-07-01/text/1/epub/OEBPS/document_2/document_2.html#_Toc171750952"^^xsd:anyURI .

C2004A04997:127 a legcons:Item,
        skos:Concept,
        dcat:Resource ;
    rdfs:label "Item I127"@en-AU ;
    rdfs:comment "Subheading Note - GraphNodeID: I127"@en-AU ;
    skos:definition "Subheading Note"@en-AU ;
    skos:narrower C2004A04997:56 ;
    skos:prefLabel "Item I127"@en-AU ;
    dcat:accessURL "https://www.legislation.gov.au/C2004A04997/2024-07-01/2024-07-01/text/1/epub/OEBPS/document_2/document_2.html#_Toc171750953"^^xsd:anyURI .

C2004A04997:128 a legcons:Item,
        skos:Concept,
        dcat:Resource ;
    rdfs:label "Item I128"@en-AU ;
    rdfs:comment "Additional Notes - GraphNodeID: I128"@en-AU ;
    skos:definition "Additional Notes"@en-AU ;
    skos:narrower C2004A04997:56 ;
    skos:prefLabel "Item I128"@en-AU ;
    dcat:accessURL "https://www.legislation.gov.au/C2004A04997/2024-07-01/2024-07-01/text/1/epub/OEBPS/document_2/document_2.html#_Toc171750954"^^xsd:anyURI .

C2004A04997:129 a legcons:Chapter,
        skos:Concept,
        dcat:Resource ;
    rdfs:label "Chapter C129"@en-AU ;
    rdfs:comment "Chapter 23 Residues and waste from the food industries prepared animal fodder - GraphNodeID: C129"@en-AU ;
    skos:definition "Chapter 23 Residues and waste from the food industries prepared animal fodder"@en-AU ;
    skos:narrower C2004A04997:102 ;
    skos:prefLabel "Chapter C129"@en-AU ;
    dcat:accessURL "https://www.legislation.gov.au/C2004A04997/2024-07-01/2024-07-01/text/1/epub/OEBPS/document_2/document_2.html#_Toc171750955"^^xsd:anyURI .

C2004A04997:13 a legcons:Item,
        skos:Concept,
        dcat:Resource ;
    rdfs:label "Item I13"@en-AU ;
    rdfs:comment "10  Certain words etc are rates of duty - GraphNodeID: I13"@en-AU ;
    skos:definition "10  Certain words etc are rates of duty"@en-AU ;
    skos:narrower C2004A04997:2 ;
    skos:prefLabel "Item I13"@en-AU ;
    dcat:accessURL "https://www.legislation.gov.au/C2004A04997/2024-07-01/2024-07-01/text/1/epub/OEBPS/document_1/document_1.html#_Toc172806513"^^xsd:anyURI .

C2004A04997:130 a legcons:Item,
        skos:Concept,
        dcat:Resource ;
    rdfs:label "Item I130"@en-AU ;
    rdfs:comment "Note - GraphNodeID: I130"@en-AU ;
    skos:definition "Note"@en-AU ;
    skos:narrower C2004A04997:56 ;
    skos:prefLabel "Item I130"@en-AU ;
    dcat:accessURL "https://www.legislation.gov.au/C2004A04997/2024-07-01/2024-07-01/text/1/epub/OEBPS/document_2/document_2.html#_Toc171750956"^^xsd:anyURI .

C2004A04997:131 a legcons:Item,
        skos:Concept,
        dcat:Resource ;
    rdfs:label "Item I131"@en-AU ;
    rdfs:comment "Subheading Note - GraphNodeID: I131"@en-AU ;
    skos:definition "Subheading Note"@en-AU ;
    skos:narrower C2004A04997:56 ;
    skos:prefLabel "Item I131"@en-AU ;
    dcat:accessURL "https://www.legislation.gov.au/C2004A04997/2024-07-01/2024-07-01/text/1/epub/OEBPS/document_2/document_2.html#_Toc171750957"^^xsd:anyURI .

C2004A04997:132 a legcons:Chapter,
        skos:Concept,
        dcat:Resource ;
    rdfs:label "Chapter C132"@en-AU ;
    rdfs:comment "Chapter 24 Tobacco and manufactured tobacco substitutes products whether or not containing nicotine intended for inhalation without combustion other nicotine containing products intended for the intake of nicotine into the human body - GraphNodeID: C132"@en-AU ;
    skos:definition "Chapter 24 Tobacco and manufactured tobacco substitutes products whether or not containing nicotine intended for inhalation without combustion other nicotine containing products intended for the intake of nicotine into the human body"@en-AU ;
    skos:narrower C2004A04997:102 ;
    skos:prefLabel "Chapter C132"@en-AU ;
    dcat:accessURL "https://www.legislation.gov.au/C2004A04997/2024-07-01/2024-07-01/text/1/epub/OEBPS/document_2/document_2.html#_Toc171750958"^^xsd:anyURI .

C2004A04997:133 a legcons:Item,
        skos:Concept,
        dcat:Resource ;
    rdfs:label "Item I133"@en-AU ;
    rdfs:comment "Notes - GraphNodeID: I133"@en-AU ;
    skos:definition "Notes"@en-AU ;
    skos:narrower C2004A04997:56 ;
    skos:prefLabel "Item I133"@en-AU ;
    dcat:accessURL "https://www.legislation.gov.au/C2004A04997/2024-07-01/2024-07-01/text/1/epub/OEBPS/document_2/document_2.html#_Toc171750959"^^xsd:anyURI .

C2004A04997:134 a legcons:Item,
        skos:Concept,
        dcat:Resource ;
    rdfs:label "Item I134"@en-AU ;
    rdfs:comment "Subheading Note - GraphNodeID: I134"@en-AU ;
    skos:definition "Subheading Note"@en-AU ;
    skos:narrower C2004A04997:56 ;
    skos:prefLabel "Item I134"@en-AU ;
    dcat:accessURL "https://www.legislation.gov.au/C2004A04997/2024-07-01/2024-07-01/text/1/epub/OEBPS/document_2/document_2.html#_Toc171750960"^^xsd:anyURI .

C2004A04997:135 a legcons:Item,
        skos:Concept,
        dcat:Resource ;
    rdfs:label "Item I135"@en-AU ;
    rdfs:comment "Additional Notes - GraphNodeID: I135"@en-AU ;
    skos:definition "Additional Notes"@en-AU ;
    skos:narrower C2004A04997:56 ;
    skos:prefLabel "Item I135"@en-AU ;
    dcat:accessURL "https://www.legislation.gov.au/C2004A04997/2024-07-01/2024-07-01/text/1/epub/OEBPS/document_2/document_2.html#_Toc171750961"^^xsd:anyURI .

C2004A04997:136 a legcons:Item,
        skos:Concept,
        dcat:Resource ;
    rdfs:label "Item I136"@en-AU ;
    rdfs:comment "Section VMineral products - GraphNodeID: I136"@en-AU ;
    skos:definition "Section VMineral products"@en-AU ;
    skos:narrower C2004A04997:56 ;
    skos:prefLabel "Item I136"@en-AU ;
    dcat:accessURL "https://www.legislation.gov.au/C2004A04997/2024-07-01/2024-07-01/text/1/epub/OEBPS/document_2/document_2.html#_Toc171750962"^^xsd:anyURI .

C2004A04997:137 a legcons:Chapter,
        skos:Concept,
        dcat:Resource ;
    rdfs:label "Chapter C137"@en-AU ;
    rdfs:comment "Chapter 25 Salt sulphur earths and stone plastering materials lime and cement - GraphNodeID: C137"@en-AU ;
    skos:definition "Chapter 25 Salt sulphur earths and stone plastering materials lime and cement"@en-AU ;
    skos:narrower C2004A04997:102 ;
    skos:prefLabel "Chapter C137"@en-AU ;
    dcat:accessURL "https://www.legislation.gov.au/C2004A04997/2024-07-01/2024-07-01/text/1/epub/OEBPS/document_2/document_2.html#_Toc171750963"^^xsd:anyURI .

C2004A04997:138 a legcons:Item,
        skos:Concept,
        dcat:Resource ;
    rdfs:label "Item I138"@en-AU ;
    rdfs:comment "Notes - GraphNodeID: I138"@en-AU ;
    skos:definition "Notes"@en-AU ;
    skos:narrower C2004A04997:56 ;
    skos:prefLabel "Item I138"@en-AU ;
    dcat:accessURL "https://www.legislation.gov.au/C2004A04997/2024-07-01/2024-07-01/text/1/epub/OEBPS/document_2/document_2.html#_Toc171750964"^^xsd:anyURI .

C2004A04997:139 a legcons:Chapter,
        skos:Concept,
        dcat:Resource ;
    rdfs:label "Chapter C139"@en-AU ;
    rdfs:comment "Chapter 26 Ores slag and ash - GraphNodeID: C139"@en-AU ;
    skos:definition "Chapter 26 Ores slag and ash"@en-AU ;
    skos:narrower C2004A04997:102 ;
    skos:prefLabel "Chapter C139"@en-AU ;
    dcat:accessURL "https://www.legislation.gov.au/C2004A04997/2024-07-01/2024-07-01/text/1/epub/OEBPS/document_2/document_2.html#_Toc171750965"^^xsd:anyURI .

C2004A04997:14 a legcons:Item,
        skos:Concept,
        dcat:Resource ;
    rdfs:label "Item I14"@en-AU ;
    rdfs:comment "11  Rates of dutyphasing rates - GraphNodeID: I14"@en-AU ;
    skos:definition "11  Rates of dutyphasing rates"@en-AU ;
    skos:narrower C2004A04997:2 ;
    skos:prefLabel "Item I14"@en-AU ;
    dcat:accessURL "https://www.legislation.gov.au/C2004A04997/2024-07-01/2024-07-01/text/1/epub/OEBPS/document_1/document_1.html#_Toc172806514"^^xsd:anyURI .

C2004A04997:140 a legcons:Item,
        skos:Concept,
        dcat:Resource ;
    rdfs:label "Item I140"@en-AU ;
    rdfs:comment "Notes - GraphNodeID: I140"@en-AU ;
    skos:definition "Notes"@en-AU ;
    skos:narrower C2004A04997:56 ;
    skos:prefLabel "Item I140"@en-AU ;
    dcat:accessURL "https://www.legislation.gov.au/C2004A04997/2024-07-01/2024-07-01/text/1/epub/OEBPS/document_2/document_2.html#_Toc171750966"^^xsd:anyURI .

C2004A04997:141 a legcons:Item,
        skos:Concept,
        dcat:Resource ;
    rdfs:label "Item I141"@en-AU ;
    rdfs:comment "Subheading Notes - GraphNodeID: I141"@en-AU ;
    skos:definition "Subheading Notes"@en-AU ;
    skos:narrower C2004A04997:56 ;
    skos:prefLabel "Item I141"@en-AU ;
    dcat:accessURL "https://www.legislation.gov.au/C2004A04997/2024-07-01/2024-07-01/text/1/epub/OEBPS/document_2/document_2.html#_Toc171750967"^^xsd:anyURI .

C2004A04997:142 a legcons:Chapter,
        skos:Concept,
        dcat:Resource ;
    rdfs:label "Chapter C142"@en-AU ;
    rdfs:comment "Chapter 27 Mineral fuels mineral oils and products of their distillation bituminous substances mineral waxes - GraphNodeID: C142"@en-AU ;
    skos:definition "Chapter 27 Mineral fuels mineral oils and products of their distillation bituminous substances mineral waxes"@en-AU ;
    skos:narrower C2004A04997:102 ;
    skos:prefLabel "Chapter C142"@en-AU ;
    dcat:accessURL "https://www.legislation.gov.au/C2004A04997/2024-07-01/2024-07-01/text/1/epub/OEBPS/document_2/document_2.html#_Toc171750968"^^xsd:anyURI .

C2004A04997:143 a legcons:Item,
        skos:Concept,
        dcat:Resource ;
    rdfs:label "Item I143"@en-AU ;
    rdfs:comment "Notes - GraphNodeID: I143"@en-AU ;
    skos:definition "Notes"@en-AU ;
    skos:narrower C2004A04997:56 ;
    skos:prefLabel "Item I143"@en-AU ;
    dcat:accessURL "https://www.legislation.gov.au/C2004A04997/2024-07-01/2024-07-01/text/1/epub/OEBPS/document_2/document_2.html#_Toc171750969"^^xsd:anyURI .

C2004A04997:144 a legcons:Item,
        skos:Concept,
        dcat:Resource ;
    rdfs:label "Item I144"@en-AU ;
    rdfs:comment "Subheading Notes - GraphNodeID: I144"@en-AU ;
    skos:definition "Subheading Notes"@en-AU ;
    skos:narrower C2004A04997:56 ;
    skos:prefLabel "Item I144"@en-AU ;
    dcat:accessURL "https://www.legislation.gov.au/C2004A04997/2024-07-01/2024-07-01/text/1/epub/OEBPS/document_2/document_2.html#_Toc171750970"^^xsd:anyURI .

C2004A04997:145 a legcons:Item,
        skos:Concept,
        dcat:Resource ;
    rdfs:label "Item I145"@en-AU ;
    rdfs:comment "Additional Notes - GraphNodeID: I145"@en-AU ;
    skos:definition "Additional Notes"@en-AU ;
    skos:narrower C2004A04997:56 ;
    skos:prefLabel "Item I145"@en-AU ;
    dcat:accessURL "https://www.legislation.gov.au/C2004A04997/2024-07-01/2024-07-01/text/1/epub/OEBPS/document_2/document_2.html#_Toc171750971"^^xsd:anyURI .

C2004A04997:146 a legcons:Item,
        skos:Concept,
        dcat:Resource ;
    rdfs:label "Item I146"@en-AU ;
    rdfs:comment "Section VIProducts of the chemical or allied industries - GraphNodeID: I146"@en-AU ;
    skos:definition "Section VIProducts of the chemical or allied industries"@en-AU ;
    skos:narrower C2004A04997:56 ;
    skos:prefLabel "Item I146"@en-AU ;
    dcat:accessURL "https://www.legislation.gov.au/C2004A04997/2024-07-01/2024-07-01/text/1/epub/OEBPS/document_2/document_2.html#_Toc171750972"^^xsd:anyURI .

C2004A04997:147 a legcons:Item,
        skos:Concept,
        dcat:Resource ;
    rdfs:label "Item I147"@en-AU ;
    rdfs:comment "Notes - GraphNodeID: I147"@en-AU ;
    skos:definition "Notes"@en-AU ;
    skos:narrower C2004A04997:56 ;
    skos:prefLabel "Item I147"@en-AU ;
    dcat:accessURL "https://www.legislation.gov.au/C2004A04997/2024-07-01/2024-07-01/text/1/epub/OEBPS/document_2/document_2.html#_Toc171750973"^^xsd:anyURI .

C2004A04997:148 a legcons:Chapter,
        skos:Concept,
        dcat:Resource ;
    rdfs:label "Chapter C148"@en-AU ;
    rdfs:comment "Chapter 28 Inorganic chemicals organic or inorganic compounds of precious metals of rare earth metals of radioactive elements or of isotopes - GraphNodeID: C148"@en-AU ;
    skos:definition "Chapter 28 Inorganic chemicals organic or inorganic compounds of precious metals of rare earth metals of radioactive elements or of isotopes"@en-AU ;
    skos:narrower C2004A04997:102 ;
    skos:prefLabel "Chapter C148"@en-AU ;
    dcat:accessURL "https://www.legislation.gov.au/C2004A04997/2024-07-01/2024-07-01/text/1/epub/OEBPS/document_2/document_2.html#_Toc171750974"^^xsd:anyURI .

C2004A04997:149 a legcons:Item,
        skos:Concept,
        dcat:Resource ;
    rdfs:label "Item I149"@en-AU ;
    rdfs:comment "Notes - GraphNodeID: I149"@en-AU ;
    skos:definition "Notes"@en-AU ;
    skos:narrower C2004A04997:56 ;
    skos:prefLabel "Item I149"@en-AU ;
    dcat:accessURL "https://www.legislation.gov.au/C2004A04997/2024-07-01/2024-07-01/text/1/epub/OEBPS/document_2/document_2.html#_Toc171750975"^^xsd:anyURI .

C2004A04997:15 a legcons:Item,
        skos:Concept,
        dcat:Resource ;
    rdfs:label "Item I15"@en-AU ;
    rdfs:comment "12  Classes of countries and places in relation to which special rates apply - GraphNodeID: I15"@en-AU ;
    skos:definition "12  Classes of countries and places in relation to which special rates apply"@en-AU ;
    skos:narrower C2004A04997:2 ;
    skos:prefLabel "Item I15"@en-AU ;
    dcat:accessURL "https://www.legislation.gov.au/C2004A04997/2024-07-01/2024-07-01/text/1/epub/OEBPS/document_1/document_1.html#_Toc172806515"^^xsd:anyURI .

C2004A04997:150 a legcons:Item,
        skos:Concept,
        dcat:Resource ;
    rdfs:label "Item I150"@en-AU ;
    rdfs:comment "Subheading Note - GraphNodeID: I150"@en-AU ;
    skos:definition "Subheading Note"@en-AU ;
    skos:narrower C2004A04997:56 ;
    skos:prefLabel "Item I150"@en-AU ;
    dcat:accessURL "https://www.legislation.gov.au/C2004A04997/2024-07-01/2024-07-01/text/1/epub/OEBPS/document_2/document_2.html#_Toc171750976"^^xsd:anyURI .

C2004A04997:151 a legcons:Item,
        skos:Concept,
        dcat:Resource ;
    rdfs:label "Item I151"@en-AU ;
    rdfs:comment "Additional Note - GraphNodeID: I151"@en-AU ;
    skos:definition "Additional Note"@en-AU ;
    skos:narrower C2004A04997:56 ;
    skos:prefLabel "Item I151"@en-AU ;
    dcat:accessURL "https://www.legislation.gov.au/C2004A04997/2024-07-01/2024-07-01/text/1/epub/OEBPS/document_2/document_2.html#_Toc171750977"^^xsd:anyURI .

C2004A04997:152 a legcons:Item,
        skos:Concept,
        dcat:Resource ;
    rdfs:label "Item I152"@en-AU ;
    rdfs:comment "Sub Chapter IChemical elements - GraphNodeID: I152"@en-AU ;
    skos:definition "Sub Chapter IChemical elements"@en-AU ;
    skos:narrower C2004A04997:56 ;
    skos:prefLabel "Item I152"@en-AU ;
    dcat:accessURL "https://www.legislation.gov.au/C2004A04997/2024-07-01/2024-07-01/text/1/epub/OEBPS/document_2/document_2.html#_Toc171750978"^^xsd:anyURI .

C2004A04997:153 a legcons:Item,
        skos:Concept,
        dcat:Resource ;
    rdfs:label "Item I153"@en-AU ;
    rdfs:comment "Sub Chapter IIInorganic acids and inorganic oxygen compounds of non metals - GraphNodeID: I153"@en-AU ;
    skos:definition "Sub Chapter IIInorganic acids and inorganic oxygen compounds of non metals"@en-AU ;
    skos:narrower C2004A04997:56 ;
    skos:prefLabel "Item I153"@en-AU ;
    dcat:accessURL "https://www.legislation.gov.au/C2004A04997/2024-07-01/2024-07-01/text/1/epub/OEBPS/document_2/document_2.html#_Toc171750979"^^xsd:anyURI .

C2004A04997:154 a legcons:Item,
        skos:Concept,
        dcat:Resource ;
    rdfs:label "Item I154"@en-AU ;
    rdfs:comment "Sub Chapter IIIHalogen or sulphur compounds of non metals - GraphNodeID: I154"@en-AU ;
    skos:definition "Sub Chapter IIIHalogen or sulphur compounds of non metals"@en-AU ;
    skos:narrower C2004A04997:56 ;
    skos:prefLabel "Item I154"@en-AU ;
    dcat:accessURL "https://www.legislation.gov.au/C2004A04997/2024-07-01/2024-07-01/text/1/epub/OEBPS/document_2/document_2.html#_Toc171750980"^^xsd:anyURI .

C2004A04997:155 a legcons:Item,
        skos:Concept,
        dcat:Resource ;
    rdfs:label "Item I155"@en-AU ;
    rdfs:comment "Sub Chapter IVInorganic bases and oxides hydroxides and peroxides of metal - GraphNodeID: I155"@en-AU ;
    skos:definition "Sub Chapter IVInorganic bases and oxides hydroxides and peroxides of metal"@en-AU ;
    skos:narrower C2004A04997:56 ;
    skos:prefLabel "Item I155"@en-AU ;
    dcat:accessURL "https://www.legislation.gov.au/C2004A04997/2024-07-01/2024-07-01/text/1/epub/OEBPS/document_2/document_2.html#_Toc171750981"^^xsd:anyURI .

C2004A04997:156 a legcons:Item,
        skos:Concept,
        dcat:Resource ;
    rdfs:label "Item I156"@en-AU ;
    rdfs:comment "Sub Chapter VSalts and peroxysalts of inorganic acids and metals - GraphNodeID: I156"@en-AU ;
    skos:definition "Sub Chapter VSalts and peroxysalts of inorganic acids and metals"@en-AU ;
    skos:narrower C2004A04997:56 ;
    skos:prefLabel "Item I156"@en-AU ;
    dcat:accessURL "https://www.legislation.gov.au/C2004A04997/2024-07-01/2024-07-01/text/1/epub/OEBPS/document_2/document_2.html#_Toc171750982"^^xsd:anyURI .

C2004A04997:157 a legcons:Item,
        skos:Concept,
        dcat:Resource ;
    rdfs:label "Item I157"@en-AU ;
    rdfs:comment "Sub Chapter VIMiscellaneous - GraphNodeID: I157"@en-AU ;
    skos:definition "Sub Chapter VIMiscellaneous"@en-AU ;
    skos:narrower C2004A04997:56 ;
    skos:prefLabel "Item I157"@en-AU ;
    dcat:accessURL "https://www.legislation.gov.au/C2004A04997/2024-07-01/2024-07-01/text/1/epub/OEBPS/document_2/document_2.html#_Toc171750983"^^xsd:anyURI .

C2004A04997:158 a legcons:Chapter,
        skos:Concept,
        dcat:Resource ;
    rdfs:label "Chapter C158"@en-AU ;
    rdfs:comment "Chapter 29 Organic chemicals - GraphNodeID: C158"@en-AU ;
    skos:definition "Chapter 29 Organic chemicals"@en-AU ;
    skos:narrower C2004A04997:102 ;
    skos:prefLabel "Chapter C158"@en-AU ;
    dcat:accessURL "https://www.legislation.gov.au/C2004A04997/2024-07-01/2024-07-01/text/1/epub/OEBPS/document_2/document_2.html#_Toc171750984"^^xsd:anyURI .

C2004A04997:159 a legcons:Item,
        skos:Concept,
        dcat:Resource ;
    rdfs:label "Item I159"@en-AU ;
    rdfs:comment "Notes - GraphNodeID: I159"@en-AU ;
    skos:definition "Notes"@en-AU ;
    skos:narrower C2004A04997:56 ;
    skos:prefLabel "Item I159"@en-AU ;
    dcat:accessURL "https://www.legislation.gov.au/C2004A04997/2024-07-01/2024-07-01/text/1/epub/OEBPS/document_2/document_2.html#_Toc171750985"^^xsd:anyURI .

C2004A04997:16 a legcons:Item,
        skos:Concept,
        dcat:Resource ;
    rdfs:label "Item I16"@en-AU ;
    rdfs:comment "13  When goods are the produce or manufacture of a particular country or place - GraphNodeID: I16"@en-AU ;
    skos:definition "13  When goods are the produce or manufacture of a particular country or place"@en-AU ;
    skos:narrower C2004A04997:2 ;
    skos:prefLabel "Item I16"@en-AU ;
    dcat:accessURL "https://www.legislation.gov.au/C2004A04997/2024-07-01/2024-07-01/text/1/epub/OEBPS/document_1/document_1.html#_Toc172806516"^^xsd:anyURI .

C2004A04997:160 a legcons:Item,
        skos:Concept,
        dcat:Resource ;
    rdfs:label "Item I160"@en-AU ;
    rdfs:comment "Subheading Notes - GraphNodeID: I160"@en-AU ;
    skos:definition "Subheading Notes"@en-AU ;
    skos:narrower C2004A04997:56 ;
    skos:prefLabel "Item I160"@en-AU ;
    dcat:accessURL "https://www.legislation.gov.au/C2004A04997/2024-07-01/2024-07-01/text/1/epub/OEBPS/document_2/document_2.html#_Toc171750986"^^xsd:anyURI .

C2004A04997:161 a legcons:Item,
        skos:Concept,
        dcat:Resource ;
    rdfs:label "Item I161"@en-AU ;
    rdfs:comment "Additional Note - GraphNodeID: I161"@en-AU ;
    skos:definition "Additional Note"@en-AU ;
    skos:narrower C2004A04997:56 ;
    skos:prefLabel "Item I161"@en-AU ;
    dcat:accessURL "https://www.legislation.gov.au/C2004A04997/2024-07-01/2024-07-01/text/1/epub/OEBPS/document_2/document_2.html#_Toc171750987"^^xsd:anyURI .

C2004A04997:162 a legcons:Item,
        skos:Concept,
        dcat:Resource ;
    rdfs:label "Item I162"@en-AU ;
    rdfs:comment "Sub Chapter IHydrocarbons and their halogenated sulphonated nitrated or nitrosated derivatives - GraphNodeID: I162"@en-AU ;
    skos:definition "Sub Chapter IHydrocarbons and their halogenated sulphonated nitrated or nitrosated derivatives"@en-AU ;
    skos:narrower C2004A04997:56 ;
    skos:prefLabel "Item I162"@en-AU ;
    dcat:accessURL "https://www.legislation.gov.au/C2004A04997/2024-07-01/2024-07-01/text/1/epub/OEBPS/document_2/document_2.html#_Toc171750988"^^xsd:anyURI .

C2004A04997:163 a legcons:Item,
        skos:Concept,
        dcat:Resource ;
    rdfs:label "Item I163"@en-AU ;
    rdfs:comment "Sub Chapter IIAlcohols and their halogenated sulphonated nitrated or nitrosated derivatives - GraphNodeID: I163"@en-AU ;
    skos:definition "Sub Chapter IIAlcohols and their halogenated sulphonated nitrated or nitrosated derivatives"@en-AU ;
    skos:narrower C2004A04997:56 ;
    skos:prefLabel "Item I163"@en-AU ;
    dcat:accessURL "https://www.legislation.gov.au/C2004A04997/2024-07-01/2024-07-01/text/1/epub/OEBPS/document_2/document_2.html#_Toc171750989"^^xsd:anyURI .

C2004A04997:164 a legcons:Item,
        skos:Concept,
        dcat:Resource ;
    rdfs:label "Item I164"@en-AU ;
    rdfs:comment "Sub Chapter IIIPhenols phenol alcohols and their halogenated sulphonated nitrated or nitrosated derivatives - GraphNodeID: I164"@en-AU ;
    skos:definition "Sub Chapter IIIPhenols phenol alcohols and their halogenated sulphonated nitrated or nitrosated derivatives"@en-AU ;
    skos:narrower C2004A04997:56 ;
    skos:prefLabel "Item I164"@en-AU ;
    dcat:accessURL "https://www.legislation.gov.au/C2004A04997/2024-07-01/2024-07-01/text/1/epub/OEBPS/document_2/document_2.html#_Toc171750990"^^xsd:anyURI .

C2004A04997:165 a legcons:Item,
        skos:Concept,
        dcat:Resource ;
    rdfs:label "Item I165"@en-AU ;
    rdfs:comment "Sub Chapter IVEthers alcohol peroxides ether peroxides acetal and hemiacetal peroxides ketone peroxides epoxides with a three membered ring acetals and hemiacetals and their halogenated sulphonated nitrated or nitrosated derivatives - GraphNodeID: I165"@en-AU ;
    skos:definition "Sub Chapter IVEthers alcohol peroxides ether peroxides acetal and hemiacetal peroxides ketone peroxides epoxides with a three membered ring acetals and hemiacetals and their halogenated sulphonated nitrated or nitrosated derivatives"@en-AU ;
    skos:narrower C2004A04997:56 ;
    skos:prefLabel "Item I165"@en-AU ;
    dcat:accessURL "https://www.legislation.gov.au/C2004A04997/2024-07-01/2024-07-01/text/1/epub/OEBPS/document_2/document_2.html#_Toc171750991"^^xsd:anyURI .

C2004A04997:166 a legcons:Item,
        skos:Concept,
        dcat:Resource ;
    rdfs:label "Item I166"@en-AU ;
    rdfs:comment "Sub Chapter VAldehyde function compounds - GraphNodeID: I166"@en-AU ;
    skos:definition "Sub Chapter VAldehyde function compounds"@en-AU ;
    skos:narrower C2004A04997:56 ;
    skos:prefLabel "Item I166"@en-AU ;
    dcat:accessURL "https://www.legislation.gov.au/C2004A04997/2024-07-01/2024-07-01/text/1/epub/OEBPS/document_2/document_2.html#_Toc171750992"^^xsd:anyURI .

C2004A04997:167 a legcons:Item,
        skos:Concept,
        dcat:Resource ;
    rdfs:label "Item I167"@en-AU ;
    rdfs:comment "Sub Chapter VIKetone function compounds and quinone function compounds - GraphNodeID: I167"@en-AU ;
    skos:definition "Sub Chapter VIKetone function compounds and quinone function compounds"@en-AU ;
    skos:narrower C2004A04997:56 ;
    skos:prefLabel "Item I167"@en-AU ;
    dcat:accessURL "https://www.legislation.gov.au/C2004A04997/2024-07-01/2024-07-01/text/1/epub/OEBPS/document_2/document_2.html#_Toc171750993"^^xsd:anyURI .

C2004A04997:168 a legcons:Item,
        skos:Concept,
        dcat:Resource ;
    rdfs:label "Item I168"@en-AU ;
    rdfs:comment "Sub Chapter VIICarboxylic acids and their anhydrides halides peroxides and peroxyacids and their halogenated sulphonated nitrated or nitrosated derivatives - GraphNodeID: I168"@en-AU ;
    skos:definition "Sub Chapter VIICarboxylic acids and their anhydrides halides peroxides and peroxyacids and their halogenated sulphonated nitrated or nitrosated derivatives"@en-AU ;
    skos:narrower C2004A04997:56 ;
    skos:prefLabel "Item I168"@en-AU ;
    dcat:accessURL "https://www.legislation.gov.au/C2004A04997/2024-07-01/2024-07-01/text/1/epub/OEBPS/document_2/document_2.html#_Toc171750994"^^xsd:anyURI .

C2004A04997:169 a legcons:Item,
        skos:Concept,
        dcat:Resource ;
    rdfs:label "Item I169"@en-AU ;
    rdfs:comment "Sub Chapter VIIIEsters of inorganic acids of non metals and their salts and their halogenated sulphonated nitrated or nitrosated derivatives - GraphNodeID: I169"@en-AU ;
    skos:definition "Sub Chapter VIIIEsters of inorganic acids of non metals and their salts and their halogenated sulphonated nitrated or nitrosated derivatives"@en-AU ;
    skos:narrower C2004A04997:56 ;
    skos:prefLabel "Item I169"@en-AU ;
    dcat:accessURL "https://www.legislation.gov.au/C2004A04997/2024-07-01/2024-07-01/text/1/epub/OEBPS/document_2/document_2.html#_Toc171750995"^^xsd:anyURI .

C2004A04997:17 a legcons:Item,
        skos:Concept,
        dcat:Resource ;
    rdfs:label "Item I17"@en-AU ;
    rdfs:comment "13 AA  When goods are Singaporean originating goods - GraphNodeID: I17"@en-AU ;
    skos:definition "13 AA  When goods are Singaporean originating goods"@en-AU ;
    skos:narrower C2004A04997:2 ;
    skos:prefLabel "Item I17"@en-AU ;
    dcat:accessURL "https://www.legislation.gov.au/C2004A04997/2024-07-01/2024-07-01/text/1/epub/OEBPS/document_1/document_1.html#_Toc172806517"^^xsd:anyURI .

C2004A04997:170 a legcons:Item,
        skos:Concept,
        dcat:Resource ;
    rdfs:label "Item I170"@en-AU ;
    rdfs:comment "Sub Chapter IXNitrogen function compounds - GraphNodeID: I170"@en-AU ;
    skos:definition "Sub Chapter IXNitrogen function compounds"@en-AU ;
    skos:narrower C2004A04997:56 ;
    skos:prefLabel "Item I170"@en-AU ;
    dcat:accessURL "https://www.legislation.gov.au/C2004A04997/2024-07-01/2024-07-01/text/1/epub/OEBPS/document_2/document_2.html#_Toc171750996"^^xsd:anyURI .

C2004A04997:171 a legcons:Item,
        skos:Concept,
        dcat:Resource ;
    rdfs:label "Item I171"@en-AU ;
    rdfs:comment "Sub Chapter XOrgano inorganic compounds heterocyclic compounds nucleic acids and their salts and sulphonamides - GraphNodeID: I171"@en-AU ;
    skos:definition "Sub Chapter XOrgano inorganic compounds heterocyclic compounds nucleic acids and their salts and sulphonamides"@en-AU ;
    skos:narrower C2004A04997:56 ;
    skos:prefLabel "Item I171"@en-AU ;
    dcat:accessURL "https://www.legislation.gov.au/C2004A04997/2024-07-01/2024-07-01/text/1/epub/OEBPS/document_2/document_2.html#_Toc171750997"^^xsd:anyURI .

C2004A04997:172 a legcons:Item,
        skos:Concept,
        dcat:Resource ;
    rdfs:label "Item I172"@en-AU ;
    rdfs:comment "Sub Chapter XIProvitamins vitamins and hormones - GraphNodeID: I172"@en-AU ;
    skos:definition "Sub Chapter XIProvitamins vitamins and hormones"@en-AU ;
    skos:narrower C2004A04997:56 ;
    skos:prefLabel "Item I172"@en-AU ;
    dcat:accessURL "https://www.legislation.gov.au/C2004A04997/2024-07-01/2024-07-01/text/1/epub/OEBPS/document_2/document_2.html#_Toc171750998"^^xsd:anyURI .

C2004A04997:173 a legcons:Item,
        skos:Concept,
        dcat:Resource ;
    rdfs:label "Item I173"@en-AU ;
    rdfs:comment "Sub Chapter XIIGlycosides and alkaloids natural or reproduced by synthesis and their salts ethers esters and other derivatives - GraphNodeID: I173"@en-AU ;
    skos:definition "Sub Chapter XIIGlycosides and alkaloids natural or reproduced by synthesis and their salts ethers esters and other derivatives"@en-AU ;
    skos:narrower C2004A04997:56 ;
    skos:prefLabel "Item I173"@en-AU ;
    dcat:accessURL "https://www.legislation.gov.au/C2004A04997/2024-07-01/2024-07-01/text/1/epub/OEBPS/document_2/document_2.html#_Toc171750999"^^xsd:anyURI .

C2004A04997:174 a legcons:Item,
        skos:Concept,
        dcat:Resource ;
    rdfs:label "Item I174"@en-AU ;
    rdfs:comment "Sub Chapter XIIIOther organic compounds - GraphNodeID: I174"@en-AU ;
    skos:definition "Sub Chapter XIIIOther organic compounds"@en-AU ;
    skos:narrower C2004A04997:56 ;
    skos:prefLabel "Item I174"@en-AU ;
    dcat:accessURL "https://www.legislation.gov.au/C2004A04997/2024-07-01/2024-07-01/text/1/epub/OEBPS/document_2/document_2.html#_Toc171751000"^^xsd:anyURI .

C2004A04997:175 a legcons:Chapter,
        skos:Concept,
        dcat:Resource ;
    rdfs:label "Chapter C175"@en-AU ;
    rdfs:comment "Chapter 30 Pharmaceutical products - GraphNodeID: C175"@en-AU ;
    skos:definition "Chapter 30 Pharmaceutical products"@en-AU ;
    skos:narrower C2004A04997:102 ;
    skos:prefLabel "Chapter C175"@en-AU ;
    dcat:accessURL "https://www.legislation.gov.au/C2004A04997/2024-07-01/2024-07-01/text/1/epub/OEBPS/document_2/document_2.html#_Toc171751001"^^xsd:anyURI .

C2004A04997:176 a legcons:Item,
        skos:Concept,
        dcat:Resource ;
    rdfs:label "Item I176"@en-AU ;
    rdfs:comment "Notes - GraphNodeID: I176"@en-AU ;
    skos:definition "Notes"@en-AU ;
    skos:narrower C2004A04997:56 ;
    skos:prefLabel "Item I176"@en-AU ;
    dcat:accessURL "https://www.legislation.gov.au/C2004A04997/2024-07-01/2024-07-01/text/1/epub/OEBPS/document_2/document_2.html#_Toc171751002"^^xsd:anyURI .

C2004A04997:177 a legcons:Item,
        skos:Concept,
        dcat:Resource ;
    rdfs:label "Item I177"@en-AU ;
    rdfs:comment "Subheading Notes - GraphNodeID: I177"@en-AU ;
    skos:definition "Subheading Notes"@en-AU ;
    skos:narrower C2004A04997:56 ;
    skos:prefLabel "Item I177"@en-AU ;
    dcat:accessURL "https://www.legislation.gov.au/C2004A04997/2024-07-01/2024-07-01/text/1/epub/OEBPS/document_2/document_2.html#_Toc171751003"^^xsd:anyURI .

C2004A04997:178 a legcons:Item,
        skos:Concept,
        dcat:Resource ;
    rdfs:label "Item I178"@en-AU ;
    rdfs:comment "Additional Notes - GraphNodeID: I178"@en-AU ;
    skos:definition "Additional Notes"@en-AU ;
    skos:narrower C2004A04997:56 ;
    skos:prefLabel "Item I178"@en-AU ;
    dcat:accessURL "https://www.legislation.gov.au/C2004A04997/2024-07-01/2024-07-01/text/1/epub/OEBPS/document_2/document_2.html#_Toc171751004"^^xsd:anyURI .

C2004A04997:179 a legcons:Chapter,
        skos:Concept,
        dcat:Resource ;
    rdfs:label "Chapter C179"@en-AU ;
    rdfs:comment "Chapter 31 Fertilisers - GraphNodeID: C179"@en-AU ;
    skos:definition "Chapter 31 Fertilisers"@en-AU ;
    skos:narrower C2004A04997:102 ;
    skos:prefLabel "Chapter C179"@en-AU ;
    dcat:accessURL "https://www.legislation.gov.au/C2004A04997/2024-07-01/2024-07-01/text/1/epub/OEBPS/document_2/document_2.html#_Toc171751005"^^xsd:anyURI .

C2004A04997:18 a legcons:Item,
        skos:Concept,
        dcat:Resource ;
    rdfs:label "Item I18"@en-AU ;
    rdfs:comment "13 A  When goods are US originating goods - GraphNodeID: I18"@en-AU ;
    skos:definition "13 A  When goods are US originating goods"@en-AU ;
    skos:narrower C2004A04997:2 ;
    skos:prefLabel "Item I18"@en-AU ;
    dcat:accessURL "https://www.legislation.gov.au/C2004A04997/2024-07-01/2024-07-01/text/1/epub/OEBPS/document_1/document_1.html#_Toc172806518"^^xsd:anyURI .

C2004A04997:180 a legcons:Item,
        skos:Concept,
        dcat:Resource ;
    rdfs:label "Item I180"@en-AU ;
    rdfs:comment "Notes - GraphNodeID: I180"@en-AU ;
    skos:definition "Notes"@en-AU ;
    skos:narrower C2004A04997:56 ;
    skos:prefLabel "Item I180"@en-AU ;
    dcat:accessURL "https://www.legislation.gov.au/C2004A04997/2024-07-01/2024-07-01/text/1/epub/OEBPS/document_2/document_2.html#_Toc171751006"^^xsd:anyURI .

C2004A04997:181 a legcons:Chapter,
        skos:Concept,
        dcat:Resource ;
    rdfs:label "Chapter C181"@en-AU ;
    rdfs:comment "Chapter 32 Tanning or dyeing extracts tannins and their derivatives dyes pigments and other colouring matter paints and varnishes putty and other mastics inks - GraphNodeID: C181"@en-AU ;
    skos:definition "Chapter 32 Tanning or dyeing extracts tannins and their derivatives dyes pigments and other colouring matter paints and varnishes putty and other mastics inks"@en-AU ;
    skos:narrower C2004A04997:102 ;
    skos:prefLabel "Chapter C181"@en-AU ;
    dcat:accessURL "https://www.legislation.gov.au/C2004A04997/2024-07-01/2024-07-01/text/1/epub/OEBPS/document_2/document_2.html#_Toc171751007"^^xsd:anyURI .

C2004A04997:182 a legcons:Item,
        skos:Concept,
        dcat:Resource ;
    rdfs:label "Item I182"@en-AU ;
    rdfs:comment "Notes - GraphNodeID: I182"@en-AU ;
    skos:definition "Notes"@en-AU ;
    skos:narrower C2004A04997:56 ;
    skos:prefLabel "Item I182"@en-AU ;
    dcat:accessURL "https://www.legislation.gov.au/C2004A04997/2024-07-01/2024-07-01/text/1/epub/OEBPS/document_2/document_2.html#_Toc171751008"^^xsd:anyURI .

C2004A04997:183 a legcons:Chapter,
        skos:Concept,
        dcat:Resource ;
    rdfs:label "Chapter C183"@en-AU ;
    rdfs:comment "Chapter 33 Essential oils and resinoids perfumery cosmetic or toilet preparations - GraphNodeID: C183"@en-AU ;
    skos:definition "Chapter 33 Essential oils and resinoids perfumery cosmetic or toilet preparations"@en-AU ;
    skos:narrower C2004A04997:102 ;
    skos:prefLabel "Chapter C183"@en-AU ;
    dcat:accessURL "https://www.legislation.gov.au/C2004A04997/2024-07-01/2024-07-01/text/1/epub/OEBPS/document_2/document_2.html#_Toc171751009"^^xsd:anyURI .

C2004A04997:184 a legcons:Item,
        skos:Concept,
        dcat:Resource ;
    rdfs:label "Item I184"@en-AU ;
    rdfs:comment "Notes - GraphNodeID: I184"@en-AU ;
    skos:definition "Notes"@en-AU ;
    skos:narrower C2004A04997:56 ;
    skos:prefLabel "Item I184"@en-AU ;
    dcat:accessURL "https://www.legislation.gov.au/C2004A04997/2024-07-01/2024-07-01/text/1/epub/OEBPS/document_2/document_2.html#_Toc171751010"^^xsd:anyURI .

C2004A04997:185 a legcons:Chapter,
        skos:Concept,
        dcat:Resource ;
    rdfs:label "Chapter C185"@en-AU ;
    rdfs:comment "Chapter 34 Soap organic surface active agents washing preparations lubricating preparations artificial waxes prepared waxes polishing or scouring preparations candles and similar articles modelling pastes dental waxes and dental preparations with a basis of plaster - GraphNodeID: C185"@en-AU ;
    skos:definition "Chapter 34 Soap organic surface active agents washing preparations lubricating preparations artificial waxes prepared waxes polishing or scouring preparations candles and similar articles modelling pastes dental waxes and dental preparations with a basis of plaster"@en-AU ;
    skos:narrower C2004A04997:102 ;
    skos:prefLabel "Chapter C185"@en-AU ;
    dcat:accessURL "https://www.legislation.gov.au/C2004A04997/2024-07-01/2024-07-01/text/1/epub/OEBPS/document_2/document_2.html#_Toc171751011"^^xsd:anyURI .

C2004A04997:186 a legcons:Item,
        skos:Concept,
        dcat:Resource ;
    rdfs:label "Item I186"@en-AU ;
    rdfs:comment "Notes - GraphNodeID: I186"@en-AU ;
    skos:definition "Notes"@en-AU ;
    skos:narrower C2004A04997:56 ;
    skos:prefLabel "Item I186"@en-AU ;
    dcat:accessURL "https://www.legislation.gov.au/C2004A04997/2024-07-01/2024-07-01/text/1/epub/OEBPS/document_2/document_2.html#_Toc171751012"^^xsd:anyURI .

C2004A04997:187 a legcons:Chapter,
        skos:Concept,
        dcat:Resource ;
    rdfs:label "Chapter C187"@en-AU ;
    rdfs:comment "Chapter 35 Albuminoidal substances modified starches glues enzymes - GraphNodeID: C187"@en-AU ;
    skos:definition "Chapter 35 Albuminoidal substances modified starches glues enzymes"@en-AU ;
    skos:narrower C2004A04997:102 ;
    skos:prefLabel "Chapter C187"@en-AU ;
    dcat:accessURL "https://www.legislation.gov.au/C2004A04997/2024-07-01/2024-07-01/text/1/epub/OEBPS/document_2/document_2.html#_Toc171751013"^^xsd:anyURI .

C2004A04997:188 a legcons:Item,
        skos:Concept,
        dcat:Resource ;
    rdfs:label "Item I188"@en-AU ;
    rdfs:comment "Notes - GraphNodeID: I188"@en-AU ;
    skos:definition "Notes"@en-AU ;
    skos:narrower C2004A04997:56 ;
    skos:prefLabel "Item I188"@en-AU ;
    dcat:accessURL "https://www.legislation.gov.au/C2004A04997/2024-07-01/2024-07-01/text/1/epub/OEBPS/document_2/document_2.html#_Toc171751014"^^xsd:anyURI .

C2004A04997:189 a legcons:Chapter,
        skos:Concept,
        dcat:Resource ;
    rdfs:label "Chapter C189"@en-AU ;
    rdfs:comment "Chapter 36 Explosives pyrotechnic products matches pyrophoric alloys certain combustible preparations - GraphNodeID: C189"@en-AU ;
    skos:definition "Chapter 36 Explosives pyrotechnic products matches pyrophoric alloys certain combustible preparations"@en-AU ;
    skos:narrower C2004A04997:102 ;
    skos:prefLabel "Chapter C189"@en-AU ;
    dcat:accessURL "https://www.legislation.gov.au/C2004A04997/2024-07-01/2024-07-01/text/1/epub/OEBPS/document_2/document_2.html#_Toc171751015"^^xsd:anyURI .

C2004A04997:19 a legcons:Item,
        skos:Concept,
        dcat:Resource ;
    rdfs:label "Item I19"@en-AU ;
    rdfs:comment "13 B  When goods are Thai originating goods - GraphNodeID: I19"@en-AU ;
    skos:definition "13 B  When goods are Thai originating goods"@en-AU ;
    skos:narrower C2004A04997:2 ;
    skos:prefLabel "Item I19"@en-AU ;
    dcat:accessURL "https://www.legislation.gov.au/C2004A04997/2024-07-01/2024-07-01/text/1/epub/OEBPS/document_1/document_1.html#_Toc172806519"^^xsd:anyURI .

C2004A04997:190 a legcons:Item,
        skos:Concept,
        dcat:Resource ;
    rdfs:label "Item I190"@en-AU ;
    rdfs:comment "Notes - GraphNodeID: I190"@en-AU ;
    skos:definition "Notes"@en-AU ;
    skos:narrower C2004A04997:56 ;
    skos:prefLabel "Item I190"@en-AU ;
    dcat:accessURL "https://www.legislation.gov.au/C2004A04997/2024-07-01/2024-07-01/text/1/epub/OEBPS/document_2/document_2.html#_Toc171751016"^^xsd:anyURI .

C2004A04997:191 a legcons:Chapter,
        skos:Concept,
        dcat:Resource ;
    rdfs:label "Chapter C191"@en-AU ;
    rdfs:comment "Chapter 37 Photographic or cinematographic goods - GraphNodeID: C191"@en-AU ;
    skos:definition "Chapter 37 Photographic or cinematographic goods"@en-AU ;
    skos:narrower C2004A04997:102 ;
    skos:prefLabel "Chapter C191"@en-AU ;
    dcat:accessURL "https://www.legislation.gov.au/C2004A04997/2024-07-01/2024-07-01/text/1/epub/OEBPS/document_2/document_2.html#_Toc171751017"^^xsd:anyURI .

C2004A04997:192 a legcons:Item,
        skos:Concept,
        dcat:Resource ;
    rdfs:label "Item I192"@en-AU ;
    rdfs:comment "Notes - GraphNodeID: I192"@en-AU ;
    skos:definition "Notes"@en-AU ;
    skos:narrower C2004A04997:56 ;
    skos:prefLabel "Item I192"@en-AU ;
    dcat:accessURL "https://www.legislation.gov.au/C2004A04997/2024-07-01/2024-07-01/text/1/epub/OEBPS/document_2/document_2.html#_Toc171751018"^^xsd:anyURI .

C2004A04997:193 a legcons:Chapter,
        skos:Concept,
        dcat:Resource ;
    rdfs:label "Chapter C193"@en-AU ;
    rdfs:comment "Chapter 38 Miscellaneous chemical products - GraphNodeID: C193"@en-AU ;
    skos:definition "Chapter 38 Miscellaneous chemical products"@en-AU ;
    skos:narrower C2004A04997:102 ;
    skos:prefLabel "Chapter C193"@en-AU ;
    dcat:accessURL "https://www.legislation.gov.au/C2004A04997/2024-07-01/2024-07-01/text/1/epub/OEBPS/document_2/document_2.html#_Toc171751019"^^xsd:anyURI .

C2004A04997:194 a legcons:Item,
        skos:Concept,
        dcat:Resource ;
    rdfs:label "Item I194"@en-AU ;
    rdfs:comment "Notes - GraphNodeID: I194"@en-AU ;
    skos:definition "Notes"@en-AU ;
    skos:narrower C2004A04997:56 ;
    skos:prefLabel "Item I194"@en-AU ;
    dcat:accessURL "https://www.legislation.gov.au/C2004A04997/2024-07-01/2024-07-01/text/1/epub/OEBPS/document_2/document_2.html#_Toc171751020"^^xsd:anyURI .

C2004A04997:195 a legcons:Item,
        skos:Concept,
        dcat:Resource ;
    rdfs:label "Item I195"@en-AU ;
    rdfs:comment "Subheading Notes - GraphNodeID: I195"@en-AU ;
    skos:definition "Subheading Notes"@en-AU ;
    skos:narrower C2004A04997:56 ;
    skos:prefLabel "Item I195"@en-AU ;
    dcat:accessURL "https://www.legislation.gov.au/C2004A04997/2024-07-01/2024-07-01/text/1/epub/OEBPS/document_2/document_2.html#_Toc171751021"^^xsd:anyURI .

C2004A04997:196 a legcons:Item,
        skos:Concept,
        dcat:Resource ;
    rdfs:label "Item I196"@en-AU ;
    rdfs:comment "Additional Note - GraphNodeID: I196"@en-AU ;
    skos:definition "Additional Note"@en-AU ;
    skos:narrower C2004A04997:56 ;
    skos:prefLabel "Item I196"@en-AU ;
    dcat:accessURL "https://www.legislation.gov.au/C2004A04997/2024-07-01/2024-07-01/text/1/epub/OEBPS/document_2/document_2.html#_Toc171751022"^^xsd:anyURI .

C2004A04997:198 a legcons:Item,
        skos:Concept,
        dcat:Resource ;
    rdfs:label "Item I198"@en-AU ;
    rdfs:comment "Schedule 3 Classification of goods and general and special rates of duty - GraphNodeID: I198"@en-AU ;
    skos:definition "Schedule 3 Classification of goods and general and special rates of duty"@en-AU ;
    skos:narrower C2004A04997:56 ;
    skos:prefLabel "Item I198"@en-AU ;
    dcat:accessURL "https://www.legislation.gov.au/C2004A04997/2024-07-01/2024-07-01/text/1/epub/OEBPS/document_3/document_3.html#_Toc171751528"^^xsd:anyURI .

C2004A04997:199 a legcons:Item,
        skos:Concept,
        dcat:Resource ;
    rdfs:label "Item I199"@en-AU ;
    rdfs:comment "Section VIIPlastics and articles thereof rubber and articles thereof - GraphNodeID: I199"@en-AU ;
    skos:definition "Section VIIPlastics and articles thereof rubber and articles thereof"@en-AU ;
    skos:narrower C2004A04997:56 ;
    skos:prefLabel "Item I199"@en-AU ;
    dcat:accessURL "https://www.legislation.gov.au/C2004A04997/2024-07-01/2024-07-01/text/1/epub/OEBPS/document_3/document_3.html#_Toc171751529"^^xsd:anyURI .

C2004A04997:20 a legcons:Item,
        skos:Concept,
        dcat:Resource ;
    rdfs:label "Item I20"@en-AU ;
    rdfs:comment "13 C  When goods are New Zealand originating goods - GraphNodeID: I20"@en-AU ;
    skos:definition "13 C  When goods are New Zealand originating goods"@en-AU ;
    skos:narrower C2004A04997:2 ;
    skos:prefLabel "Item I20"@en-AU ;
    dcat:accessURL "https://www.legislation.gov.au/C2004A04997/2024-07-01/2024-07-01/text/1/epub/OEBPS/document_1/document_1.html#_Toc172806520"^^xsd:anyURI .

C2004A04997:200 a legcons:Item,
        skos:Concept,
        dcat:Resource ;
    rdfs:label "Item I200"@en-AU ;
    rdfs:comment "Notes - GraphNodeID: I200"@en-AU ;
    skos:definition "Notes"@en-AU ;
    skos:narrower C2004A04997:56 ;
    skos:prefLabel "Item I200"@en-AU ;
    dcat:accessURL "https://www.legislation.gov.au/C2004A04997/2024-07-01/2024-07-01/text/1/epub/OEBPS/document_3/document_3.html#_Toc171751530"^^xsd:anyURI .

C2004A04997:201 a legcons:Item,
        skos:Concept,
        dcat:Resource ;
    rdfs:label "Item I201"@en-AU ;
    rdfs:comment "Additional Note - GraphNodeID: I201"@en-AU ;
    skos:definition "Additional Note"@en-AU ;
    skos:narrower C2004A04997:56 ;
    skos:prefLabel "Item I201"@en-AU ;
    dcat:accessURL "https://www.legislation.gov.au/C2004A04997/2024-07-01/2024-07-01/text/1/epub/OEBPS/document_3/document_3.html#_Toc171751531"^^xsd:anyURI .

C2004A04997:202 a legcons:Chapter,
        skos:Concept,
        dcat:Resource ;
    rdfs:label "Chapter C202"@en-AU ;
    rdfs:comment "Chapter 39 Plastics and articles thereof - GraphNodeID: C202"@en-AU ;
    skos:definition "Chapter 39 Plastics and articles thereof"@en-AU ;
    skos:narrower C2004A04997:197 ;
    skos:prefLabel "Chapter C202"@en-AU ;
    dcat:accessURL "https://www.legislation.gov.au/C2004A04997/2024-07-01/2024-07-01/text/1/epub/OEBPS/document_3/document_3.html#_Toc171751532"^^xsd:anyURI .

C2004A04997:203 a legcons:Item,
        skos:Concept,
        dcat:Resource ;
    rdfs:label "Item I203"@en-AU ;
    rdfs:comment "Notes - GraphNodeID: I203"@en-AU ;
    skos:definition "Notes"@en-AU ;
    skos:narrower C2004A04997:56 ;
    skos:prefLabel "Item I203"@en-AU ;
    dcat:accessURL "https://www.legislation.gov.au/C2004A04997/2024-07-01/2024-07-01/text/1/epub/OEBPS/document_3/document_3.html#_Toc171751533"^^xsd:anyURI .

C2004A04997:204 a legcons:Item,
        skos:Concept,
        dcat:Resource ;
    rdfs:label "Item I204"@en-AU ;
    rdfs:comment "Subheading Notes - GraphNodeID: I204"@en-AU ;
    skos:definition "Subheading Notes"@en-AU ;
    skos:narrower C2004A04997:56 ;
    skos:prefLabel "Item I204"@en-AU ;
    dcat:accessURL "https://www.legislation.gov.au/C2004A04997/2024-07-01/2024-07-01/text/1/epub/OEBPS/document_3/document_3.html#_Toc171751534"^^xsd:anyURI .

C2004A04997:205 a legcons:Item,
        skos:Concept,
        dcat:Resource ;
    rdfs:label "Item I205"@en-AU ;
    rdfs:comment "Additional Notes - GraphNodeID: I205"@en-AU ;
    skos:definition "Additional Notes"@en-AU ;
    skos:narrower C2004A04997:56 ;
    skos:prefLabel "Item I205"@en-AU ;
    dcat:accessURL "https://www.legislation.gov.au/C2004A04997/2024-07-01/2024-07-01/text/1/epub/OEBPS/document_3/document_3.html#_Toc171751535"^^xsd:anyURI .

C2004A04997:206 a legcons:Item,
        skos:Concept,
        dcat:Resource ;
    rdfs:label "Item I206"@en-AU ;
    rdfs:comment "Sub Chapter IPrimary forms - GraphNodeID: I206"@en-AU ;
    skos:definition "Sub Chapter IPrimary forms"@en-AU ;
    skos:narrower C2004A04997:56 ;
    skos:prefLabel "Item I206"@en-AU ;
    dcat:accessURL "https://www.legislation.gov.au/C2004A04997/2024-07-01/2024-07-01/text/1/epub/OEBPS/document_3/document_3.html#_Toc171751536"^^xsd:anyURI .

C2004A04997:207 a legcons:Item,
        skos:Concept,
        dcat:Resource ;
    rdfs:label "Item I207"@en-AU ;
    rdfs:comment "Sub Chapter IIWaste parings and scrap semi manufactures articles - GraphNodeID: I207"@en-AU ;
    skos:definition "Sub Chapter IIWaste parings and scrap semi manufactures articles"@en-AU ;
    skos:narrower C2004A04997:56 ;
    skos:prefLabel "Item I207"@en-AU ;
    dcat:accessURL "https://www.legislation.gov.au/C2004A04997/2024-07-01/2024-07-01/text/1/epub/OEBPS/document_3/document_3.html#_Toc171751537"^^xsd:anyURI .

C2004A04997:208 a legcons:Chapter,
        skos:Concept,
        dcat:Resource ;
    rdfs:label "Chapter C208"@en-AU ;
    rdfs:comment "Chapter 40 Rubber and articles thereof - GraphNodeID: C208"@en-AU ;
    skos:definition "Chapter 40 Rubber and articles thereof"@en-AU ;
    skos:narrower C2004A04997:197 ;
    skos:prefLabel "Chapter C208"@en-AU ;
    dcat:accessURL "https://www.legislation.gov.au/C2004A04997/2024-07-01/2024-07-01/text/1/epub/OEBPS/document_3/document_3.html#_Toc171751538"^^xsd:anyURI .

C2004A04997:209 a legcons:Item,
        skos:Concept,
        dcat:Resource ;
    rdfs:label "Item I209"@en-AU ;
    rdfs:comment "Notes - GraphNodeID: I209"@en-AU ;
    skos:definition "Notes"@en-AU ;
    skos:narrower C2004A04997:56 ;
    skos:prefLabel "Item I209"@en-AU ;
    dcat:accessURL "https://www.legislation.gov.au/C2004A04997/2024-07-01/2024-07-01/text/1/epub/OEBPS/document_3/document_3.html#_Toc171751539"^^xsd:anyURI .

C2004A04997:21 a legcons:Item,
        skos:Concept,
        dcat:Resource ;
    rdfs:label "Item I21"@en-AU ;
    rdfs:comment "13 CA  When goods are Peruvian originating goods - GraphNodeID: I21"@en-AU ;
    skos:definition "13 CA  When goods are Peruvian originating goods"@en-AU ;
    skos:narrower C2004A04997:2 ;
    skos:prefLabel "Item I21"@en-AU ;
    dcat:accessURL "https://www.legislation.gov.au/C2004A04997/2024-07-01/2024-07-01/text/1/epub/OEBPS/document_1/document_1.html#_Toc172806521"^^xsd:anyURI .

C2004A04997:210 a legcons:Item,
        skos:Concept,
        dcat:Resource ;
    rdfs:label "Item I210"@en-AU ;
    rdfs:comment "Section VIIIRaw hides and skins leather furskins and articles thereof saddlery and harness travel goods handbags and similar containers articles of animal gut other than silk worm gut - GraphNodeID: I210"@en-AU ;
    skos:definition "Section VIIIRaw hides and skins leather furskins and articles thereof saddlery and harness travel goods handbags and similar containers articles of animal gut other than silk worm gut"@en-AU ;
    skos:narrower C2004A04997:56 ;
    skos:prefLabel "Item I210"@en-AU ;
    dcat:accessURL "https://www.legislation.gov.au/C2004A04997/2024-07-01/2024-07-01/text/1/epub/OEBPS/document_3/document_3.html#_Toc171751540"^^xsd:anyURI .

C2004A04997:211 a legcons:Chapter,
        skos:Concept,
        dcat:Resource ;
    rdfs:label "Chapter C211"@en-AU ;
    rdfs:comment "Chapter 41 Raw hides and skins other than furskins and leather - GraphNodeID: C211"@en-AU ;
    skos:definition "Chapter 41 Raw hides and skins other than furskins and leather"@en-AU ;
    skos:narrower C2004A04997:197 ;
    skos:prefLabel "Chapter C211"@en-AU ;
    dcat:accessURL "https://www.legislation.gov.au/C2004A04997/2024-07-01/2024-07-01/text/1/epub/OEBPS/document_3/document_3.html#_Toc171751541"^^xsd:anyURI .

C2004A04997:212 a legcons:Item,
        skos:Concept,
        dcat:Resource ;
    rdfs:label "Item I212"@en-AU ;
    rdfs:comment "Notes - GraphNodeID: I212"@en-AU ;
    skos:definition "Notes"@en-AU ;
    skos:narrower C2004A04997:56 ;
    skos:prefLabel "Item I212"@en-AU ;
    dcat:accessURL "https://www.legislation.gov.au/C2004A04997/2024-07-01/2024-07-01/text/1/epub/OEBPS/document_3/document_3.html#_Toc171751542"^^xsd:anyURI .

C2004A04997:213 a legcons:Chapter,
        skos:Concept,
        dcat:Resource ;
    rdfs:label "Chapter C213"@en-AU ;
    rdfs:comment "Chapter 42 Articles of leather saddlery and harness travel goods handbags and similar containers articles of animal gut other than silk worm gut - GraphNodeID: C213"@en-AU ;
    skos:definition "Chapter 42 Articles of leather saddlery and harness travel goods handbags and similar containers articles of animal gut other than silk worm gut"@en-AU ;
    skos:narrower C2004A04997:197 ;
    skos:prefLabel "Chapter C213"@en-AU ;
    dcat:accessURL "https://www.legislation.gov.au/C2004A04997/2024-07-01/2024-07-01/text/1/epub/OEBPS/document_3/document_3.html#_Toc171751543"^^xsd:anyURI .

C2004A04997:214 a legcons:Item,
        skos:Concept,
        dcat:Resource ;
    rdfs:label "Item I214"@en-AU ;
    rdfs:comment "Notes - GraphNodeID: I214"@en-AU ;
    skos:definition "Notes"@en-AU ;
    skos:narrower C2004A04997:56 ;
    skos:prefLabel "Item I214"@en-AU ;
    dcat:accessURL "https://www.legislation.gov.au/C2004A04997/2024-07-01/2024-07-01/text/1/epub/OEBPS/document_3/document_3.html#_Toc171751544"^^xsd:anyURI .

C2004A04997:215 a legcons:Chapter,
        skos:Concept,
        dcat:Resource ;
    rdfs:label "Chapter C215"@en-AU ;
    rdfs:comment "Chapter 43 Furskins and artificial fur manufactures thereof - GraphNodeID: C215"@en-AU ;
    skos:definition "Chapter 43 Furskins and artificial fur manufactures thereof"@en-AU ;
    skos:narrower C2004A04997:197 ;
    skos:prefLabel "Chapter C215"@en-AU ;
    dcat:accessURL "https://www.legislation.gov.au/C2004A04997/2024-07-01/2024-07-01/text/1/epub/OEBPS/document_3/document_3.html#_Toc171751545"^^xsd:anyURI .

C2004A04997:216 a legcons:Item,
        skos:Concept,
        dcat:Resource ;
    rdfs:label "Item I216"@en-AU ;
    rdfs:comment "Notes - GraphNodeID: I216"@en-AU ;
    skos:definition "Notes"@en-AU ;
    skos:narrower C2004A04997:56 ;
    skos:prefLabel "Item I216"@en-AU ;
    dcat:accessURL "https://www.legislation.gov.au/C2004A04997/2024-07-01/2024-07-01/text/1/epub/OEBPS/document_3/document_3.html#_Toc171751546"^^xsd:anyURI .

C2004A04997:217 a legcons:Item,
        skos:Concept,
        dcat:Resource ;
    rdfs:label "Item I217"@en-AU ;
    rdfs:comment "Section IXWood and articles of wood wood charcoal cork and articles of cork manufactures of straw of esparto or of other plaiting materials basketware and wickerwork - GraphNodeID: I217"@en-AU ;
    skos:definition "Section IXWood and articles of wood wood charcoal cork and articles of cork manufactures of straw of esparto or of other plaiting materials basketware and wickerwork"@en-AU ;
    skos:narrower C2004A04997:56 ;
    skos:prefLabel "Item I217"@en-AU ;
    dcat:accessURL "https://www.legislation.gov.au/C2004A04997/2024-07-01/2024-07-01/text/1/epub/OEBPS/document_3/document_3.html#_Toc171751547"^^xsd:anyURI .

C2004A04997:218 a legcons:Chapter,
        skos:Concept,
        dcat:Resource ;
    rdfs:label "Chapter C218"@en-AU ;
    rdfs:comment "Chapter 44 Wood and articles of wood wood charcoal - GraphNodeID: C218"@en-AU ;
    skos:definition "Chapter 44 Wood and articles of wood wood charcoal"@en-AU ;
    skos:narrower C2004A04997:197 ;
    skos:prefLabel "Chapter C218"@en-AU ;
    dcat:accessURL "https://www.legislation.gov.au/C2004A04997/2024-07-01/2024-07-01/text/1/epub/OEBPS/document_3/document_3.html#_Toc171751548"^^xsd:anyURI .

C2004A04997:219 a legcons:Item,
        skos:Concept,
        dcat:Resource ;
    rdfs:label "Item I219"@en-AU ;
    rdfs:comment "Notes - GraphNodeID: I219"@en-AU ;
    skos:definition "Notes"@en-AU ;
    skos:narrower C2004A04997:56 ;
    skos:prefLabel "Item I219"@en-AU ;
    dcat:accessURL "https://www.legislation.gov.au/C2004A04997/2024-07-01/2024-07-01/text/1/epub/OEBPS/document_3/document_3.html#_Toc171751549"^^xsd:anyURI .

C2004A04997:22 a legcons:Item,
        skos:Concept,
        dcat:Resource ;
    rdfs:label "Item I22"@en-AU ;
    rdfs:comment "13 D  When goods are Chilean originating goods - GraphNodeID: I22"@en-AU ;
    skos:definition "13 D  When goods are Chilean originating goods"@en-AU ;
    skos:narrower C2004A04997:2 ;
    skos:prefLabel "Item I22"@en-AU ;
    dcat:accessURL "https://www.legislation.gov.au/C2004A04997/2024-07-01/2024-07-01/text/1/epub/OEBPS/document_1/document_1.html#_Toc172806522"^^xsd:anyURI .

C2004A04997:220 a legcons:Item,
        skos:Concept,
        dcat:Resource ;
    rdfs:label "Item I220"@en-AU ;
    rdfs:comment "Subheading Notes - GraphNodeID: I220"@en-AU ;
    skos:definition "Subheading Notes"@en-AU ;
    skos:narrower C2004A04997:56 ;
    skos:prefLabel "Item I220"@en-AU ;
    dcat:accessURL "https://www.legislation.gov.au/C2004A04997/2024-07-01/2024-07-01/text/1/epub/OEBPS/document_3/document_3.html#_Toc171751550"^^xsd:anyURI .

C2004A04997:221 a legcons:Item,
        skos:Concept,
        dcat:Resource ;
    rdfs:label "Item I221"@en-AU ;
    rdfs:comment "Additional Notes - GraphNodeID: I221"@en-AU ;
    skos:definition "Additional Notes"@en-AU ;
    skos:narrower C2004A04997:56 ;
    skos:prefLabel "Item I221"@en-AU ;
    dcat:accessURL "https://www.legislation.gov.au/C2004A04997/2024-07-01/2024-07-01/text/1/epub/OEBPS/document_3/document_3.html#_Toc171751551"^^xsd:anyURI .

C2004A04997:222 a legcons:Chapter,
        skos:Concept,
        dcat:Resource ;
    rdfs:label "Chapter C222"@en-AU ;
    rdfs:comment "Chapter 45 Cork and articles of cork - GraphNodeID: C222"@en-AU ;
    skos:definition "Chapter 45 Cork and articles of cork"@en-AU ;
    skos:narrower C2004A04997:197 ;
    skos:prefLabel "Chapter C222"@en-AU ;
    dcat:accessURL "https://www.legislation.gov.au/C2004A04997/2024-07-01/2024-07-01/text/1/epub/OEBPS/document_3/document_3.html#_Toc171751552"^^xsd:anyURI .

C2004A04997:223 a legcons:Item,
        skos:Concept,
        dcat:Resource ;
    rdfs:label "Item I223"@en-AU ;
    rdfs:comment "Note - GraphNodeID: I223"@en-AU ;
    skos:definition "Note"@en-AU ;
    skos:narrower C2004A04997:56 ;
    skos:prefLabel "Item I223"@en-AU ;
    dcat:accessURL "https://www.legislation.gov.au/C2004A04997/2024-07-01/2024-07-01/text/1/epub/OEBPS/document_3/document_3.html#_Toc171751553"^^xsd:anyURI .

C2004A04997:224 a legcons:Chapter,
        skos:Concept,
        dcat:Resource ;
    rdfs:label "Chapter C224"@en-AU ;
    rdfs:comment "Chapter 46 Manufactures of straw of esparto or of other plaiting materials basketware and wickerwork - GraphNodeID: C224"@en-AU ;
    skos:definition "Chapter 46 Manufactures of straw of esparto or of other plaiting materials basketware and wickerwork"@en-AU ;
    skos:narrower C2004A04997:197 ;
    skos:prefLabel "Chapter C224"@en-AU ;
    dcat:accessURL "https://www.legislation.gov.au/C2004A04997/2024-07-01/2024-07-01/text/1/epub/OEBPS/document_3/document_3.html#_Toc171751554"^^xsd:anyURI .

C2004A04997:225 a legcons:Item,
        skos:Concept,
        dcat:Resource ;
    rdfs:label "Item I225"@en-AU ;
    rdfs:comment "Notes - GraphNodeID: I225"@en-AU ;
    skos:definition "Notes"@en-AU ;
    skos:narrower C2004A04997:56 ;
    skos:prefLabel "Item I225"@en-AU ;
    dcat:accessURL "https://www.legislation.gov.au/C2004A04997/2024-07-01/2024-07-01/text/1/epub/OEBPS/document_3/document_3.html#_Toc171751555"^^xsd:anyURI .

C2004A04997:226 a legcons:Item,
        skos:Concept,
        dcat:Resource ;
    rdfs:label "Item I226"@en-AU ;
    rdfs:comment "Section XPulp of wood or of other fibrous cellulosic material recovered waste and scrap paper or paperboard paper and paperboard and articles thereof - GraphNodeID: I226"@en-AU ;
    skos:definition "Section XPulp of wood or of other fibrous cellulosic material recovered waste and scrap paper or paperboard paper and paperboard and articles thereof"@en-AU ;
    skos:narrower C2004A04997:56 ;
    skos:prefLabel "Item I226"@en-AU ;
    dcat:accessURL "https://www.legislation.gov.au/C2004A04997/2024-07-01/2024-07-01/text/1/epub/OEBPS/document_3/document_3.html#_Toc171751556"^^xsd:anyURI .

C2004A04997:227 a legcons:Chapter,
        skos:Concept,
        dcat:Resource ;
    rdfs:label "Chapter C227"@en-AU ;
    rdfs:comment "Chapter 47 Pulp of wood or of other fibrous cellulosic material recovered waste and scrap paper or paperboard - GraphNodeID: C227"@en-AU ;
    skos:definition "Chapter 47 Pulp of wood or of other fibrous cellulosic material recovered waste and scrap paper or paperboard"@en-AU ;
    skos:narrower C2004A04997:197 ;
    skos:prefLabel "Chapter C227"@en-AU ;
    dcat:accessURL "https://www.legislation.gov.au/C2004A04997/2024-07-01/2024-07-01/text/1/epub/OEBPS/document_3/document_3.html#_Toc171751557"^^xsd:anyURI .

C2004A04997:228 a legcons:Item,
        skos:Concept,
        dcat:Resource ;
    rdfs:label "Item I228"@en-AU ;
    rdfs:comment "Note - GraphNodeID: I228"@en-AU ;
    skos:definition "Note"@en-AU ;
    skos:narrower C2004A04997:56 ;
    skos:prefLabel "Item I228"@en-AU ;
    dcat:accessURL "https://www.legislation.gov.au/C2004A04997/2024-07-01/2024-07-01/text/1/epub/OEBPS/document_3/document_3.html#_Toc171751558"^^xsd:anyURI .

C2004A04997:229 a legcons:Chapter,
        skos:Concept,
        dcat:Resource ;
    rdfs:label "Chapter C229"@en-AU ;
    rdfs:comment "Chapter 48 Paper and paperboard articles of paper pulp of paper or of paperboard - GraphNodeID: C229"@en-AU ;
    skos:definition "Chapter 48 Paper and paperboard articles of paper pulp of paper or of paperboard"@en-AU ;
    skos:narrower C2004A04997:197 ;
    skos:prefLabel "Chapter C229"@en-AU ;
    dcat:accessURL "https://www.legislation.gov.au/C2004A04997/2024-07-01/2024-07-01/text/1/epub/OEBPS/document_3/document_3.html#_Toc171751559"^^xsd:anyURI .

C2004A04997:23 a legcons:Item,
        skos:Concept,
        dcat:Resource ;
    rdfs:label "Item I23"@en-AU ;
    rdfs:comment "13 E  When goods are ASEAN Australia New Zealand AANZ originating goods - GraphNodeID: I23"@en-AU ;
    skos:definition "13 E  When goods are ASEAN Australia New Zealand AANZ originating goods"@en-AU ;
    skos:narrower C2004A04997:2 ;
    skos:prefLabel "Item I23"@en-AU ;
    dcat:accessURL "https://www.legislation.gov.au/C2004A04997/2024-07-01/2024-07-01/text/1/epub/OEBPS/document_1/document_1.html#_Toc172806523"^^xsd:anyURI .

C2004A04997:230 a legcons:Item,
        skos:Concept,
        dcat:Resource ;
    rdfs:label "Item I230"@en-AU ;
    rdfs:comment "Notes - GraphNodeID: I230"@en-AU ;
    skos:definition "Notes"@en-AU ;
    skos:narrower C2004A04997:56 ;
    skos:prefLabel "Item I230"@en-AU ;
    dcat:accessURL "https://www.legislation.gov.au/C2004A04997/2024-07-01/2024-07-01/text/1/epub/OEBPS/document_3/document_3.html#_Toc171751560"^^xsd:anyURI .

C2004A04997:231 a legcons:Item,
        skos:Concept,
        dcat:Resource ;
    rdfs:label "Item I231"@en-AU ;
    rdfs:comment "Subheading Notes - GraphNodeID: I231"@en-AU ;
    skos:definition "Subheading Notes"@en-AU ;
    skos:narrower C2004A04997:56 ;
    skos:prefLabel "Item I231"@en-AU ;
    dcat:accessURL "https://www.legislation.gov.au/C2004A04997/2024-07-01/2024-07-01/text/1/epub/OEBPS/document_3/document_3.html#_Toc171751561"^^xsd:anyURI .

C2004A04997:232 a legcons:Item,
        skos:Concept,
        dcat:Resource ;
    rdfs:label "Item I232"@en-AU ;
    rdfs:comment "Additional Notes - GraphNodeID: I232"@en-AU ;
    skos:definition "Additional Notes"@en-AU ;
    skos:narrower C2004A04997:56 ;
    skos:prefLabel "Item I232"@en-AU ;
    dcat:accessURL "https://www.legislation.gov.au/C2004A04997/2024-07-01/2024-07-01/text/1/epub/OEBPS/document_3/document_3.html#_Toc171751562"^^xsd:anyURI .

C2004A04997:233 a legcons:Chapter,
        skos:Concept,
        dcat:Resource ;
    rdfs:label "Chapter C233"@en-AU ;
    rdfs:comment "Chapter 49 Printed books newspapers pictures and other products of the printing industry manuscripts typescripts and plans - GraphNodeID: C233"@en-AU ;
    skos:definition "Chapter 49 Printed books newspapers pictures and other products of the printing industry manuscripts typescripts and plans"@en-AU ;
    skos:narrower C2004A04997:197 ;
    skos:prefLabel "Chapter C233"@en-AU ;
    dcat:accessURL "https://www.legislation.gov.au/C2004A04997/2024-07-01/2024-07-01/text/1/epub/OEBPS/document_3/document_3.html#_Toc171751563"^^xsd:anyURI .

C2004A04997:234 a legcons:Item,
        skos:Concept,
        dcat:Resource ;
    rdfs:label "Item I234"@en-AU ;
    rdfs:comment "Notes - GraphNodeID: I234"@en-AU ;
    skos:definition "Notes"@en-AU ;
    skos:narrower C2004A04997:56 ;
    skos:prefLabel "Item I234"@en-AU ;
    dcat:accessURL "https://www.legislation.gov.au/C2004A04997/2024-07-01/2024-07-01/text/1/epub/OEBPS/document_3/document_3.html#_Toc171751564"^^xsd:anyURI .

C2004A04997:235 a legcons:Item,
        skos:Concept,
        dcat:Resource ;
    rdfs:label "Item I235"@en-AU ;
    rdfs:comment "Section XITextiles and textile articles - GraphNodeID: I235"@en-AU ;
    skos:definition "Section XITextiles and textile articles"@en-AU ;
    skos:narrower C2004A04997:56 ;
    skos:prefLabel "Item I235"@en-AU ;
    dcat:accessURL "https://www.legislation.gov.au/C2004A04997/2024-07-01/2024-07-01/text/1/epub/OEBPS/document_3/document_3.html#_Toc171751565"^^xsd:anyURI .

C2004A04997:236 a legcons:Item,
        skos:Concept,
        dcat:Resource ;
    rdfs:label "Item I236"@en-AU ;
    rdfs:comment "Notes - GraphNodeID: I236"@en-AU ;
    skos:definition "Notes"@en-AU ;
    skos:narrower C2004A04997:56 ;
    skos:prefLabel "Item I236"@en-AU ;
    dcat:accessURL "https://www.legislation.gov.au/C2004A04997/2024-07-01/2024-07-01/text/1/epub/OEBPS/document_3/document_3.html#_Toc171751566"^^xsd:anyURI .

C2004A04997:237 a legcons:Item,
        skos:Concept,
        dcat:Resource ;
    rdfs:label "Item I237"@en-AU ;
    rdfs:comment "Subheading Notes - GraphNodeID: I237"@en-AU ;
    skos:definition "Subheading Notes"@en-AU ;
    skos:narrower C2004A04997:56 ;
    skos:prefLabel "Item I237"@en-AU ;
    dcat:accessURL "https://www.legislation.gov.au/C2004A04997/2024-07-01/2024-07-01/text/1/epub/OEBPS/document_3/document_3.html#_Toc171751567"^^xsd:anyURI .

C2004A04997:238 a legcons:Item,
        skos:Concept,
        dcat:Resource ;
    rdfs:label "Item I238"@en-AU ;
    rdfs:comment "Additional Notes - GraphNodeID: I238"@en-AU ;
    skos:definition "Additional Notes"@en-AU ;
    skos:narrower C2004A04997:56 ;
    skos:prefLabel "Item I238"@en-AU ;
    dcat:accessURL "https://www.legislation.gov.au/C2004A04997/2024-07-01/2024-07-01/text/1/epub/OEBPS/document_3/document_3.html#_Toc171751568"^^xsd:anyURI .

C2004A04997:239 a legcons:Chapter,
        skos:Concept,
        dcat:Resource ;
    rdfs:label "Chapter C239"@en-AU ;
    rdfs:comment "Chapter 50 Silk - GraphNodeID: C239"@en-AU ;
    skos:definition "Chapter 50 Silk"@en-AU ;
    skos:narrower C2004A04997:197 ;
    skos:prefLabel "Chapter C239"@en-AU ;
    dcat:accessURL "https://www.legislation.gov.au/C2004A04997/2024-07-01/2024-07-01/text/1/epub/OEBPS/document_3/document_3.html#_Toc171751569"^^xsd:anyURI .

C2004A04997:24 a legcons:Item,
        skos:Concept,
        dcat:Resource ;
    rdfs:label "Item I24"@en-AU ;
    rdfs:comment "13 EA  When goods are Pacific Islands originating goods - GraphNodeID: I24"@en-AU ;
    skos:definition "13 EA  When goods are Pacific Islands originating goods"@en-AU ;
    skos:narrower C2004A04997:2 ;
    skos:prefLabel "Item I24"@en-AU ;
    dcat:accessURL "https://www.legislation.gov.au/C2004A04997/2024-07-01/2024-07-01/text/1/epub/OEBPS/document_1/document_1.html#_Toc172806524"^^xsd:anyURI .

C2004A04997:240 a legcons:Chapter,
        skos:Concept,
        dcat:Resource ;
    rdfs:label "Chapter C240"@en-AU ;
    rdfs:comment "Chapter 51 Wool fine or coarse animal hair horsehair yarn and woven fabric - GraphNodeID: C240"@en-AU ;
    skos:definition "Chapter 51 Wool fine or coarse animal hair horsehair yarn and woven fabric"@en-AU ;
    skos:narrower C2004A04997:197 ;
    skos:prefLabel "Chapter C240"@en-AU ;
    dcat:accessURL "https://www.legislation.gov.au/C2004A04997/2024-07-01/2024-07-01/text/1/epub/OEBPS/document_3/document_3.html#_Toc171751570"^^xsd:anyURI .

C2004A04997:241 a legcons:Item,
        skos:Concept,
        dcat:Resource ;
    rdfs:label "Item I241"@en-AU ;
    rdfs:comment "Note - GraphNodeID: I241"@en-AU ;
    skos:definition "Note"@en-AU ;
    skos:narrower C2004A04997:56 ;
    skos:prefLabel "Item I241"@en-AU ;
    dcat:accessURL "https://www.legislation.gov.au/C2004A04997/2024-07-01/2024-07-01/text/1/epub/OEBPS/document_3/document_3.html#_Toc171751571"^^xsd:anyURI .

C2004A04997:242 a legcons:Chapter,
        skos:Concept,
        dcat:Resource ;
    rdfs:label "Chapter C242"@en-AU ;
    rdfs:comment "Chapter 52 Cotton - GraphNodeID: C242"@en-AU ;
    skos:definition "Chapter 52 Cotton"@en-AU ;
    skos:narrower C2004A04997:197 ;
    skos:prefLabel "Chapter C242"@en-AU ;
    dcat:accessURL "https://www.legislation.gov.au/C2004A04997/2024-07-01/2024-07-01/text/1/epub/OEBPS/document_3/document_3.html#_Toc171751572"^^xsd:anyURI .

C2004A04997:243 a legcons:Item,
        skos:Concept,
        dcat:Resource ;
    rdfs:label "Item I243"@en-AU ;
    rdfs:comment "Subheading Note - GraphNodeID: I243"@en-AU ;
    skos:definition "Subheading Note"@en-AU ;
    skos:narrower C2004A04997:56 ;
    skos:prefLabel "Item I243"@en-AU ;
    dcat:accessURL "https://www.legislation.gov.au/C2004A04997/2024-07-01/2024-07-01/text/1/epub/OEBPS/document_3/document_3.html#_Toc171751573"^^xsd:anyURI .

C2004A04997:244 a legcons:Chapter,
        skos:Concept,
        dcat:Resource ;
    rdfs:label "Chapter C244"@en-AU ;
    rdfs:comment "Chapter 53 Other vegetable textile fibres paper yarn and woven fabrics of paper yarn - GraphNodeID: C244"@en-AU ;
    skos:definition "Chapter 53 Other vegetable textile fibres paper yarn and woven fabrics of paper yarn"@en-AU ;
    skos:narrower C2004A04997:197 ;
    skos:prefLabel "Chapter C244"@en-AU ;
    dcat:accessURL "https://www.legislation.gov.au/C2004A04997/2024-07-01/2024-07-01/text/1/epub/OEBPS/document_3/document_3.html#_Toc171751574"^^xsd:anyURI .

C2004A04997:245 a legcons:Chapter,
        skos:Concept,
        dcat:Resource ;
    rdfs:label "Chapter C245"@en-AU ;
    rdfs:comment "Chapter 54 Man made filaments strip and the like of man made textile materials - GraphNodeID: C245"@en-AU ;
    skos:definition "Chapter 54 Man made filaments strip and the like of man made textile materials"@en-AU ;
    skos:narrower C2004A04997:197 ;
    skos:prefLabel "Chapter C245"@en-AU ;
    dcat:accessURL "https://www.legislation.gov.au/C2004A04997/2024-07-01/2024-07-01/text/1/epub/OEBPS/document_3/document_3.html#_Toc171751575"^^xsd:anyURI .

C2004A04997:246 a legcons:Item,
        skos:Concept,
        dcat:Resource ;
    rdfs:label "Item I246"@en-AU ;
    rdfs:comment "Notes - GraphNodeID: I246"@en-AU ;
    skos:definition "Notes"@en-AU ;
    skos:narrower C2004A04997:56 ;
    skos:prefLabel "Item I246"@en-AU ;
    dcat:accessURL "https://www.legislation.gov.au/C2004A04997/2024-07-01/2024-07-01/text/1/epub/OEBPS/document_3/document_3.html#_Toc171751576"^^xsd:anyURI .

C2004A04997:247 a legcons:Chapter,
        skos:Concept,
        dcat:Resource ;
    rdfs:label "Chapter C247"@en-AU ;
    rdfs:comment "Chapter 55 Man made staple fibres - GraphNodeID: C247"@en-AU ;
    skos:definition "Chapter 55 Man made staple fibres"@en-AU ;
    skos:narrower C2004A04997:197 ;
    skos:prefLabel "Chapter C247"@en-AU ;
    dcat:accessURL "https://www.legislation.gov.au/C2004A04997/2024-07-01/2024-07-01/text/1/epub/OEBPS/document_3/document_3.html#_Toc171751577"^^xsd:anyURI .

C2004A04997:248 a legcons:Item,
        skos:Concept,
        dcat:Resource ;
    rdfs:label "Item I248"@en-AU ;
    rdfs:comment "Note - GraphNodeID: I248"@en-AU ;
    skos:definition "Note"@en-AU ;
    skos:narrower C2004A04997:56 ;
    skos:prefLabel "Item I248"@en-AU ;
    dcat:accessURL "https://www.legislation.gov.au/C2004A04997/2024-07-01/2024-07-01/text/1/epub/OEBPS/document_3/document_3.html#_Toc171751578"^^xsd:anyURI .

C2004A04997:249 a legcons:Chapter,
        skos:Concept,
        dcat:Resource ;
    rdfs:label "Chapter C249"@en-AU ;
    rdfs:comment "Chapter 56 Wadding felt and nonwovens special yarns twine cordage ropes and cables and articles thereof - GraphNodeID: C249"@en-AU ;
    skos:definition "Chapter 56 Wadding felt and nonwovens special yarns twine cordage ropes and cables and articles thereof"@en-AU ;
    skos:narrower C2004A04997:197 ;
    skos:prefLabel "Chapter C249"@en-AU ;
    dcat:accessURL "https://www.legislation.gov.au/C2004A04997/2024-07-01/2024-07-01/text/1/epub/OEBPS/document_3/document_3.html#_Toc171751579"^^xsd:anyURI .

C2004A04997:25 a legcons:Item,
        skos:Concept,
        dcat:Resource ;
    rdfs:label "Item I25"@en-AU ;
    rdfs:comment "13 EB  When goods are Trans Pacific Partnership originating goods - GraphNodeID: I25"@en-AU ;
    skos:definition "13 EB  When goods are Trans Pacific Partnership originating goods"@en-AU ;
    skos:narrower C2004A04997:2 ;
    skos:prefLabel "Item I25"@en-AU ;
    dcat:accessURL "https://www.legislation.gov.au/C2004A04997/2024-07-01/2024-07-01/text/1/epub/OEBPS/document_1/document_1.html#_Toc172806525"^^xsd:anyURI .

C2004A04997:250 a legcons:Item,
        skos:Concept,
        dcat:Resource ;
    rdfs:label "Item I250"@en-AU ;
    rdfs:comment "Notes - GraphNodeID: I250"@en-AU ;
    skos:definition "Notes"@en-AU ;
    skos:narrower C2004A04997:56 ;
    skos:prefLabel "Item I250"@en-AU ;
    dcat:accessURL "https://www.legislation.gov.au/C2004A04997/2024-07-01/2024-07-01/text/1/epub/OEBPS/document_3/document_3.html#_Toc171751580"^^xsd:anyURI .

C2004A04997:251 a legcons:Chapter,
        skos:Concept,
        dcat:Resource ;
    rdfs:label "Chapter C251"@en-AU ;
    rdfs:comment "Chapter 57 Carpets and other textile floor coverings - GraphNodeID: C251"@en-AU ;
    skos:definition "Chapter 57 Carpets and other textile floor coverings"@en-AU ;
    skos:narrower C2004A04997:197 ;
    skos:prefLabel "Chapter C251"@en-AU ;
    dcat:accessURL "https://www.legislation.gov.au/C2004A04997/2024-07-01/2024-07-01/text/1/epub/OEBPS/document_3/document_3.html#_Toc171751581"^^xsd:anyURI .

C2004A04997:252 a legcons:Item,
        skos:Concept,
        dcat:Resource ;
    rdfs:label "Item I252"@en-AU ;
    rdfs:comment "Notes - GraphNodeID: I252"@en-AU ;
    skos:definition "Notes"@en-AU ;
    skos:narrower C2004A04997:56 ;
    skos:prefLabel "Item I252"@en-AU ;
    dcat:accessURL "https://www.legislation.gov.au/C2004A04997/2024-07-01/2024-07-01/text/1/epub/OEBPS/document_3/document_3.html#_Toc171751582"^^xsd:anyURI .

C2004A04997:253 a legcons:Item,
        skos:Concept,
        dcat:Resource ;
    rdfs:label "Item I253"@en-AU ;
    rdfs:comment "Additional Notes - GraphNodeID: I253"@en-AU ;
    skos:definition "Additional Notes"@en-AU ;
    skos:narrower C2004A04997:56 ;
    skos:prefLabel "Item I253"@en-AU ;
    dcat:accessURL "https://www.legislation.gov.au/C2004A04997/2024-07-01/2024-07-01/text/1/epub/OEBPS/document_3/document_3.html#_Toc171751583"^^xsd:anyURI .

C2004A04997:254 a legcons:Chapter,
        skos:Concept,
        dcat:Resource ;
    rdfs:label "Chapter C254"@en-AU ;
    rdfs:comment "Chapter 58 Special woven fabrics tufted textile fabrics lace tapestries trimmings embroidery - GraphNodeID: C254"@en-AU ;
    skos:definition "Chapter 58 Special woven fabrics tufted textile fabrics lace tapestries trimmings embroidery"@en-AU ;
    skos:narrower C2004A04997:197 ;
    skos:prefLabel "Chapter C254"@en-AU ;
    dcat:accessURL "https://www.legislation.gov.au/C2004A04997/2024-07-01/2024-07-01/text/1/epub/OEBPS/document_3/document_3.html#_Toc171751584"^^xsd:anyURI .

C2004A04997:255 a legcons:Item,
        skos:Concept,
        dcat:Resource ;
    rdfs:label "Item I255"@en-AU ;
    rdfs:comment "Notes - GraphNodeID: I255"@en-AU ;
    skos:definition "Notes"@en-AU ;
    skos:narrower C2004A04997:56 ;
    skos:prefLabel "Item I255"@en-AU ;
    dcat:accessURL "https://www.legislation.gov.au/C2004A04997/2024-07-01/2024-07-01/text/1/epub/OEBPS/document_3/document_3.html#_Toc171751585"^^xsd:anyURI .

C2004A04997:256 a legcons:Item,
        skos:Concept,
        dcat:Resource ;
    rdfs:label "Item I256"@en-AU ;
    rdfs:comment "Additional Note - GraphNodeID: I256"@en-AU ;
    skos:definition "Additional Note"@en-AU ;
    skos:narrower C2004A04997:56 ;
    skos:prefLabel "Item I256"@en-AU ;
    dcat:accessURL "https://www.legislation.gov.au/C2004A04997/2024-07-01/2024-07-01/text/1/epub/OEBPS/document_3/document_3.html#_Toc171751586"^^xsd:anyURI .

C2004A04997:257 a legcons:Chapter,
        skos:Concept,
        dcat:Resource ;
    rdfs:label "Chapter C257"@en-AU ;
    rdfs:comment "Chapter 59 Impregnated coated covered or laminated textile fabrics textile articles of a kind suitable for industrial use - GraphNodeID: C257"@en-AU ;
    skos:definition "Chapter 59 Impregnated coated covered or laminated textile fabrics textile articles of a kind suitable for industrial use"@en-AU ;
    skos:narrower C2004A04997:197 ;
    skos:prefLabel "Chapter C257"@en-AU ;
    dcat:accessURL "https://www.legislation.gov.au/C2004A04997/2024-07-01/2024-07-01/text/1/epub/OEBPS/document_3/document_3.html#_Toc171751587"^^xsd:anyURI .

C2004A04997:258 a legcons:Item,
        skos:Concept,
        dcat:Resource ;
    rdfs:label "Item I258"@en-AU ;
    rdfs:comment "Notes - GraphNodeID: I258"@en-AU ;
    skos:definition "Notes"@en-AU ;
    skos:narrower C2004A04997:56 ;
    skos:prefLabel "Item I258"@en-AU ;
    dcat:accessURL "https://www.legislation.gov.au/C2004A04997/2024-07-01/2024-07-01/text/1/epub/OEBPS/document_3/document_3.html#_Toc171751588"^^xsd:anyURI .

C2004A04997:26 a legcons:Item,
        skos:Concept,
        dcat:Resource ;
    rdfs:label "Item I26"@en-AU ;
    rdfs:comment "13 F  When goods are Malaysian originating goods - GraphNodeID: I26"@en-AU ;
    skos:definition "13 F  When goods are Malaysian originating goods"@en-AU ;
    skos:narrower C2004A04997:2 ;
    skos:prefLabel "Item I26"@en-AU ;
    dcat:accessURL "https://www.legislation.gov.au/C2004A04997/2024-07-01/2024-07-01/text/1/epub/OEBPS/document_1/document_1.html#_Toc172806526"^^xsd:anyURI .

C2004A04997:260 a legcons:Item,
        skos:Concept,
        dcat:Resource ;
    rdfs:label "Item I260"@en-AU ;
    rdfs:comment "Schedule 3 Classification of goods and general and special rates of duty - GraphNodeID: I260"@en-AU ;
    skos:definition "Schedule 3 Classification of goods and general and special rates of duty"@en-AU ;
    skos:narrower C2004A04997:56 ;
    skos:prefLabel "Item I260"@en-AU ;
    dcat:accessURL "https://www.legislation.gov.au/C2004A04997/2024-07-01/2024-07-01/text/1/epub/OEBPS/document_4/document_4.html#_Toc171751991"^^xsd:anyURI .

C2004A04997:261 a legcons:Item,
        skos:Concept,
        dcat:Resource ;
    rdfs:label "Item I261"@en-AU ;
    rdfs:comment "Section XITextiles and textile articles - GraphNodeID: I261"@en-AU ;
    skos:definition "Section XITextiles and textile articles"@en-AU ;
    skos:narrower C2004A04997:56 ;
    skos:prefLabel "Item I261"@en-AU ;
    dcat:accessURL "https://www.legislation.gov.au/C2004A04997/2024-07-01/2024-07-01/text/1/epub/OEBPS/document_4/document_4.html#_Toc171751992"^^xsd:anyURI .

C2004A04997:262 a legcons:Chapter,
        skos:Concept,
        dcat:Resource ;
    rdfs:label "Chapter C262"@en-AU ;
    rdfs:comment "Chapter 60 Knitted or crocheted fabrics - GraphNodeID: C262"@en-AU ;
    skos:definition "Chapter 60 Knitted or crocheted fabrics"@en-AU ;
    skos:narrower C2004A04997:259 ;
    skos:prefLabel "Chapter C262"@en-AU ;
    dcat:accessURL "https://www.legislation.gov.au/C2004A04997/2024-07-01/2024-07-01/text/1/epub/OEBPS/document_4/document_4.html#_Toc171751993"^^xsd:anyURI .

C2004A04997:263 a legcons:Item,
        skos:Concept,
        dcat:Resource ;
    rdfs:label "Item I263"@en-AU ;
    rdfs:comment "Notes - GraphNodeID: I263"@en-AU ;
    skos:definition "Notes"@en-AU ;
    skos:narrower C2004A04997:56 ;
    skos:prefLabel "Item I263"@en-AU ;
    dcat:accessURL "https://www.legislation.gov.au/C2004A04997/2024-07-01/2024-07-01/text/1/epub/OEBPS/document_4/document_4.html#_Toc171751994"^^xsd:anyURI .

C2004A04997:264 a legcons:Item,
        skos:Concept,
        dcat:Resource ;
    rdfs:label "Item I264"@en-AU ;
    rdfs:comment "Subheading Note - GraphNodeID: I264"@en-AU ;
    skos:definition "Subheading Note"@en-AU ;
    skos:narrower C2004A04997:56 ;
    skos:prefLabel "Item I264"@en-AU ;
    dcat:accessURL "https://www.legislation.gov.au/C2004A04997/2024-07-01/2024-07-01/text/1/epub/OEBPS/document_4/document_4.html#_Toc171751995"^^xsd:anyURI .

C2004A04997:265 a legcons:Chapter,
        skos:Concept,
        dcat:Resource ;
    rdfs:label "Chapter C265"@en-AU ;
    rdfs:comment "Chapter 61 Articles of apparel and clothing accessories knitted or crocheted - GraphNodeID: C265"@en-AU ;
    skos:definition "Chapter 61 Articles of apparel and clothing accessories knitted or crocheted"@en-AU ;
    skos:narrower C2004A04997:259 ;
    skos:prefLabel "Chapter C265"@en-AU ;
    dcat:accessURL "https://www.legislation.gov.au/C2004A04997/2024-07-01/2024-07-01/text/1/epub/OEBPS/document_4/document_4.html#_Toc171751996"^^xsd:anyURI .

C2004A04997:266 a legcons:Item,
        skos:Concept,
        dcat:Resource ;
    rdfs:label "Item I266"@en-AU ;
    rdfs:comment "Notes - GraphNodeID: I266"@en-AU ;
    skos:definition "Notes"@en-AU ;
    skos:narrower C2004A04997:56 ;
    skos:prefLabel "Item I266"@en-AU ;
    dcat:accessURL "https://www.legislation.gov.au/C2004A04997/2024-07-01/2024-07-01/text/1/epub/OEBPS/document_4/document_4.html#_Toc171751997"^^xsd:anyURI .

C2004A04997:267 a legcons:Item,
        skos:Concept,
        dcat:Resource ;
    rdfs:label "Item I267"@en-AU ;
    rdfs:comment "Additional Note - GraphNodeID: I267"@en-AU ;
    skos:definition "Additional Note"@en-AU ;
    skos:narrower C2004A04997:56 ;
    skos:prefLabel "Item I267"@en-AU ;
    dcat:accessURL "https://www.legislation.gov.au/C2004A04997/2024-07-01/2024-07-01/text/1/epub/OEBPS/document_4/document_4.html#_Toc171751998"^^xsd:anyURI .

C2004A04997:268 a legcons:Chapter,
        skos:Concept,
        dcat:Resource ;
    rdfs:label "Chapter C268"@en-AU ;
    rdfs:comment "Chapter 62 Articles of apparel and clothing accessories not knitted or crocheted - GraphNodeID: C268"@en-AU ;
    skos:definition "Chapter 62 Articles of apparel and clothing accessories not knitted or crocheted"@en-AU ;
    skos:narrower C2004A04997:259 ;
    skos:prefLabel "Chapter C268"@en-AU ;
    dcat:accessURL "https://www.legislation.gov.au/C2004A04997/2024-07-01/2024-07-01/text/1/epub/OEBPS/document_4/document_4.html#_Toc171751999"^^xsd:anyURI .

C2004A04997:269 a legcons:Item,
        skos:Concept,
        dcat:Resource ;
    rdfs:label "Item I269"@en-AU ;
    rdfs:comment "Notes - GraphNodeID: I269"@en-AU ;
    skos:definition "Notes"@en-AU ;
    skos:narrower C2004A04997:56 ;
    skos:prefLabel "Item I269"@en-AU ;
    dcat:accessURL "https://www.legislation.gov.au/C2004A04997/2024-07-01/2024-07-01/text/1/epub/OEBPS/document_4/document_4.html#_Toc171752000"^^xsd:anyURI .

C2004A04997:27 a legcons:Item,
        skos:Concept,
        dcat:Resource ;
    rdfs:label "Item I27"@en-AU ;
    rdfs:comment "13 FA  When goods are Indonesian originating goods - GraphNodeID: I27"@en-AU ;
    skos:definition "13 FA  When goods are Indonesian originating goods"@en-AU ;
    skos:narrower C2004A04997:2 ;
    skos:prefLabel "Item I27"@en-AU ;
    dcat:accessURL "https://www.legislation.gov.au/C2004A04997/2024-07-01/2024-07-01/text/1/epub/OEBPS/document_1/document_1.html#_Toc172806527"^^xsd:anyURI .

C2004A04997:270 a legcons:Item,
        skos:Concept,
        dcat:Resource ;
    rdfs:label "Item I270"@en-AU ;
    rdfs:comment "Additional Note - GraphNodeID: I270"@en-AU ;
    skos:definition "Additional Note"@en-AU ;
    skos:narrower C2004A04997:56 ;
    skos:prefLabel "Item I270"@en-AU ;
    dcat:accessURL "https://www.legislation.gov.au/C2004A04997/2024-07-01/2024-07-01/text/1/epub/OEBPS/document_4/document_4.html#_Toc171752001"^^xsd:anyURI .

C2004A04997:271 a legcons:Chapter,
        skos:Concept,
        dcat:Resource ;
    rdfs:label "Chapter C271"@en-AU ;
    rdfs:comment "Chapter 63 Other made up textile articles sets worn clothing and worn textile articles rags - GraphNodeID: C271"@en-AU ;
    skos:definition "Chapter 63 Other made up textile articles sets worn clothing and worn textile articles rags"@en-AU ;
    skos:narrower C2004A04997:259 ;
    skos:prefLabel "Chapter C271"@en-AU ;
    dcat:accessURL "https://www.legislation.gov.au/C2004A04997/2024-07-01/2024-07-01/text/1/epub/OEBPS/document_4/document_4.html#_Toc171752002"^^xsd:anyURI .

C2004A04997:272 a legcons:Item,
        skos:Concept,
        dcat:Resource ;
    rdfs:label "Item I272"@en-AU ;
    rdfs:comment "Notes - GraphNodeID: I272"@en-AU ;
    skos:definition "Notes"@en-AU ;
    skos:narrower C2004A04997:56 ;
    skos:prefLabel "Item I272"@en-AU ;
    dcat:accessURL "https://www.legislation.gov.au/C2004A04997/2024-07-01/2024-07-01/text/1/epub/OEBPS/document_4/document_4.html#_Toc171752003"^^xsd:anyURI .

C2004A04997:273 a legcons:Item,
        skos:Concept,
        dcat:Resource ;
    rdfs:label "Item I273"@en-AU ;
    rdfs:comment "Subheading Note - GraphNodeID: I273"@en-AU ;
    skos:definition "Subheading Note"@en-AU ;
    skos:narrower C2004A04997:56 ;
    skos:prefLabel "Item I273"@en-AU ;
    dcat:accessURL "https://www.legislation.gov.au/C2004A04997/2024-07-01/2024-07-01/text/1/epub/OEBPS/document_4/document_4.html#_Toc171752004"^^xsd:anyURI .

C2004A04997:274 a legcons:Item,
        skos:Concept,
        dcat:Resource ;
    rdfs:label "Item I274"@en-AU ;
    rdfs:comment "Sub Chapter IOther made up textile articles - GraphNodeID: I274"@en-AU ;
    skos:definition "Sub Chapter IOther made up textile articles"@en-AU ;
    skos:narrower C2004A04997:56 ;
    skos:prefLabel "Item I274"@en-AU ;
    dcat:accessURL "https://www.legislation.gov.au/C2004A04997/2024-07-01/2024-07-01/text/1/epub/OEBPS/document_4/document_4.html#_Toc171752005"^^xsd:anyURI .

C2004A04997:275 a legcons:Item,
        skos:Concept,
        dcat:Resource ;
    rdfs:label "Item I275"@en-AU ;
    rdfs:comment "Sub Chapter IISets - GraphNodeID: I275"@en-AU ;
    skos:definition "Sub Chapter IISets"@en-AU ;
    skos:narrower C2004A04997:56 ;
    skos:prefLabel "Item I275"@en-AU ;
    dcat:accessURL "https://www.legislation.gov.au/C2004A04997/2024-07-01/2024-07-01/text/1/epub/OEBPS/document_4/document_4.html#_Toc171752006"^^xsd:anyURI .

C2004A04997:276 a legcons:Item,
        skos:Concept,
        dcat:Resource ;
    rdfs:label "Item I276"@en-AU ;
    rdfs:comment "Sub Chapter IIIWorn clothing and worn textile articles rags - GraphNodeID: I276"@en-AU ;
    skos:definition "Sub Chapter IIIWorn clothing and worn textile articles rags"@en-AU ;
    skos:narrower C2004A04997:56 ;
    skos:prefLabel "Item I276"@en-AU ;
    dcat:accessURL "https://www.legislation.gov.au/C2004A04997/2024-07-01/2024-07-01/text/1/epub/OEBPS/document_4/document_4.html#_Toc171752007"^^xsd:anyURI .

C2004A04997:277 a legcons:Item,
        skos:Concept,
        dcat:Resource ;
    rdfs:label "Item I277"@en-AU ;
    rdfs:comment "Section XIIFootwear headgear umbrellas sun umbrellas walking sticks seat sticks whips riding crops and parts thereof prepared feathers and articles made therewith artificial flowers articles of human hair - GraphNodeID: I277"@en-AU ;
    skos:definition "Section XIIFootwear headgear umbrellas sun umbrellas walking sticks seat sticks whips riding crops and parts thereof prepared feathers and articles made therewith artificial flowers articles of human hair"@en-AU ;
    skos:narrower C2004A04997:56 ;
    skos:prefLabel "Item I277"@en-AU ;
    dcat:accessURL "https://www.legislation.gov.au/C2004A04997/2024-07-01/2024-07-01/text/1/epub/OEBPS/document_4/document_4.html#_Toc171752008"^^xsd:anyURI .

C2004A04997:278 a legcons:Chapter,
        skos:Concept,
        dcat:Resource ;
    rdfs:label "Chapter C278"@en-AU ;
    rdfs:comment "Chapter 64 Footwear gaiters and the like parts of such articles - GraphNodeID: C278"@en-AU ;
    skos:definition "Chapter 64 Footwear gaiters and the like parts of such articles"@en-AU ;
    skos:narrower C2004A04997:259 ;
    skos:prefLabel "Chapter C278"@en-AU ;
    dcat:accessURL "https://www.legislation.gov.au/C2004A04997/2024-07-01/2024-07-01/text/1/epub/OEBPS/document_4/document_4.html#_Toc171752009"^^xsd:anyURI .

C2004A04997:279 a legcons:Item,
        skos:Concept,
        dcat:Resource ;
    rdfs:label "Item I279"@en-AU ;
    rdfs:comment "Notes - GraphNodeID: I279"@en-AU ;
    skos:definition "Notes"@en-AU ;
    skos:narrower C2004A04997:56 ;
    skos:prefLabel "Item I279"@en-AU ;
    dcat:accessURL "https://www.legislation.gov.au/C2004A04997/2024-07-01/2024-07-01/text/1/epub/OEBPS/document_4/document_4.html#_Toc171752010"^^xsd:anyURI .

C2004A04997:28 a legcons:Item,
        skos:Concept,
        dcat:Resource ;
    rdfs:label "Item I28"@en-AU ;
    rdfs:comment "13 G  When goods are Korean originating goods - GraphNodeID: I28"@en-AU ;
    skos:definition "13 G  When goods are Korean originating goods"@en-AU ;
    skos:narrower C2004A04997:2 ;
    skos:prefLabel "Item I28"@en-AU ;
    dcat:accessURL "https://www.legislation.gov.au/C2004A04997/2024-07-01/2024-07-01/text/1/epub/OEBPS/document_1/document_1.html#_Toc172806528"^^xsd:anyURI .

C2004A04997:280 a legcons:Item,
        skos:Concept,
        dcat:Resource ;
    rdfs:label "Item I280"@en-AU ;
    rdfs:comment "Subheading Note - GraphNodeID: I280"@en-AU ;
    skos:definition "Subheading Note"@en-AU ;
    skos:narrower C2004A04997:56 ;
    skos:prefLabel "Item I280"@en-AU ;
    dcat:accessURL "https://www.legislation.gov.au/C2004A04997/2024-07-01/2024-07-01/text/1/epub/OEBPS/document_4/document_4.html#_Toc171752011"^^xsd:anyURI .

C2004A04997:281 a legcons:Chapter,
        skos:Concept,
        dcat:Resource ;
    rdfs:label "Chapter C281"@en-AU ;
    rdfs:comment "Chapter 65 Headgear and parts thereof - GraphNodeID: C281"@en-AU ;
    skos:definition "Chapter 65 Headgear and parts thereof"@en-AU ;
    skos:narrower C2004A04997:259 ;
    skos:prefLabel "Chapter C281"@en-AU ;
    dcat:accessURL "https://www.legislation.gov.au/C2004A04997/2024-07-01/2024-07-01/text/1/epub/OEBPS/document_4/document_4.html#_Toc171752012"^^xsd:anyURI .

C2004A04997:282 a legcons:Item,
        skos:Concept,
        dcat:Resource ;
    rdfs:label "Item I282"@en-AU ;
    rdfs:comment "Notes - GraphNodeID: I282"@en-AU ;
    skos:definition "Notes"@en-AU ;
    skos:narrower C2004A04997:56 ;
    skos:prefLabel "Item I282"@en-AU ;
    dcat:accessURL "https://www.legislation.gov.au/C2004A04997/2024-07-01/2024-07-01/text/1/epub/OEBPS/document_4/document_4.html#_Toc171752013"^^xsd:anyURI .

C2004A04997:283 a legcons:Chapter,
        skos:Concept,
        dcat:Resource ;
    rdfs:label "Chapter C283"@en-AU ;
    rdfs:comment "Chapter 66 Umbrellas sun umbrellas walking sticks seat sticks whips riding crops and parts thereof - GraphNodeID: C283"@en-AU ;
    skos:definition "Chapter 66 Umbrellas sun umbrellas walking sticks seat sticks whips riding crops and parts thereof"@en-AU ;
    skos:narrower C2004A04997:259 ;
    skos:prefLabel "Chapter C283"@en-AU ;
    dcat:accessURL "https://www.legislation.gov.au/C2004A04997/2024-07-01/2024-07-01/text/1/epub/OEBPS/document_4/document_4.html#_Toc171752014"^^xsd:anyURI .

C2004A04997:284 a legcons:Item,
        skos:Concept,
        dcat:Resource ;
    rdfs:label "Item I284"@en-AU ;
    rdfs:comment "Notes - GraphNodeID: I284"@en-AU ;
    skos:definition "Notes"@en-AU ;
    skos:narrower C2004A04997:56 ;
    skos:prefLabel "Item I284"@en-AU ;
    dcat:accessURL "https://www.legislation.gov.au/C2004A04997/2024-07-01/2024-07-01/text/1/epub/OEBPS/document_4/document_4.html#_Toc171752015"^^xsd:anyURI .

C2004A04997:285 a legcons:Chapter,
        skos:Concept,
        dcat:Resource ;
    rdfs:label "Chapter C285"@en-AU ;
    rdfs:comment "Chapter 67 Prepared feathers and down and articles made of feathers or of down artificial flowers articles of human hair - GraphNodeID: C285"@en-AU ;
    skos:definition "Chapter 67 Prepared feathers and down and articles made of feathers or of down artificial flowers articles of human hair"@en-AU ;
    skos:narrower C2004A04997:259 ;
    skos:prefLabel "Chapter C285"@en-AU ;
    dcat:accessURL "https://www.legislation.gov.au/C2004A04997/2024-07-01/2024-07-01/text/1/epub/OEBPS/document_4/document_4.html#_Toc171752016"^^xsd:anyURI .

C2004A04997:286 a legcons:Item,
        skos:Concept,
        dcat:Resource ;
    rdfs:label "Item I286"@en-AU ;
    rdfs:comment "Notes - GraphNodeID: I286"@en-AU ;
    skos:definition "Notes"@en-AU ;
    skos:narrower C2004A04997:56 ;
    skos:prefLabel "Item I286"@en-AU ;
    dcat:accessURL "https://www.legislation.gov.au/C2004A04997/2024-07-01/2024-07-01/text/1/epub/OEBPS/document_4/document_4.html#_Toc171752017"^^xsd:anyURI .

C2004A04997:287 a legcons:Item,
        skos:Concept,
        dcat:Resource ;
    rdfs:label "Item I287"@en-AU ;
    rdfs:comment "Section XIIIArticles of stone plaster cement asbestos mica or similar materials ceramic products glass and glassware - GraphNodeID: I287"@en-AU ;
    skos:definition "Section XIIIArticles of stone plaster cement asbestos mica or similar materials ceramic products glass and glassware"@en-AU ;
    skos:narrower C2004A04997:56 ;
    skos:prefLabel "Item I287"@en-AU ;
    dcat:accessURL "https://www.legislation.gov.au/C2004A04997/2024-07-01/2024-07-01/text/1/epub/OEBPS/document_4/document_4.html#_Toc171752018"^^xsd:anyURI .

C2004A04997:288 a legcons:Chapter,
        skos:Concept,
        dcat:Resource ;
    rdfs:label "Chapter C288"@en-AU ;
    rdfs:comment "Chapter 68 Articles of stone plaster cement asbestos mica or similar materials - GraphNodeID: C288"@en-AU ;
    skos:definition "Chapter 68 Articles of stone plaster cement asbestos mica or similar materials"@en-AU ;
    skos:narrower C2004A04997:259 ;
    skos:prefLabel "Chapter C288"@en-AU ;
    dcat:accessURL "https://www.legislation.gov.au/C2004A04997/2024-07-01/2024-07-01/text/1/epub/OEBPS/document_4/document_4.html#_Toc171752019"^^xsd:anyURI .

C2004A04997:289 a legcons:Item,
        skos:Concept,
        dcat:Resource ;
    rdfs:label "Item I289"@en-AU ;
    rdfs:comment "Notes - GraphNodeID: I289"@en-AU ;
    skos:definition "Notes"@en-AU ;
    skos:narrower C2004A04997:56 ;
    skos:prefLabel "Item I289"@en-AU ;
    dcat:accessURL "https://www.legislation.gov.au/C2004A04997/2024-07-01/2024-07-01/text/1/epub/OEBPS/document_4/document_4.html#_Toc171752020"^^xsd:anyURI .

C2004A04997:29 a legcons:Item,
        skos:Concept,
        dcat:Resource ;
    rdfs:label "Item I29"@en-AU ;
    rdfs:comment "13 GA  When goods are Indian originating goods - GraphNodeID: I29"@en-AU ;
    skos:definition "13 GA  When goods are Indian originating goods"@en-AU ;
    skos:narrower C2004A04997:2 ;
    skos:prefLabel "Item I29"@en-AU ;
    dcat:accessURL "https://www.legislation.gov.au/C2004A04997/2024-07-01/2024-07-01/text/1/epub/OEBPS/document_1/document_1.html#_Toc172806529"^^xsd:anyURI .

C2004A04997:290 a legcons:Chapter,
        skos:Concept,
        dcat:Resource ;
    rdfs:label "Chapter C290"@en-AU ;
    rdfs:comment "Chapter 69 Ceramic products - GraphNodeID: C290"@en-AU ;
    skos:definition "Chapter 69 Ceramic products"@en-AU ;
    skos:narrower C2004A04997:259 ;
    skos:prefLabel "Chapter C290"@en-AU ;
    dcat:accessURL "https://www.legislation.gov.au/C2004A04997/2024-07-01/2024-07-01/text/1/epub/OEBPS/document_4/document_4.html#_Toc171752021"^^xsd:anyURI .

C2004A04997:291 a legcons:Item,
        skos:Concept,
        dcat:Resource ;
    rdfs:label "Item I291"@en-AU ;
    rdfs:comment "Notes - GraphNodeID: I291"@en-AU ;
    skos:definition "Notes"@en-AU ;
    skos:narrower C2004A04997:56 ;
    skos:prefLabel "Item I291"@en-AU ;
    dcat:accessURL "https://www.legislation.gov.au/C2004A04997/2024-07-01/2024-07-01/text/1/epub/OEBPS/document_4/document_4.html#_Toc171752022"^^xsd:anyURI .

C2004A04997:292 a legcons:Item,
        skos:Concept,
        dcat:Resource ;
    rdfs:label "Item I292"@en-AU ;
    rdfs:comment "Sub Chapter IGoods of siliceous fossil meals or of similar siliceous earths and refractory goods - GraphNodeID: I292"@en-AU ;
    skos:definition "Sub Chapter IGoods of siliceous fossil meals or of similar siliceous earths and refractory goods"@en-AU ;
    skos:narrower C2004A04997:56 ;
    skos:prefLabel "Item I292"@en-AU ;
    dcat:accessURL "https://www.legislation.gov.au/C2004A04997/2024-07-01/2024-07-01/text/1/epub/OEBPS/document_4/document_4.html#_Toc171752023"^^xsd:anyURI .

C2004A04997:293 a legcons:Item,
        skos:Concept,
        dcat:Resource ;
    rdfs:label "Item I293"@en-AU ;
    rdfs:comment "Sub Chapter IIOther ceramic products - GraphNodeID: I293"@en-AU ;
    skos:definition "Sub Chapter IIOther ceramic products"@en-AU ;
    skos:narrower C2004A04997:56 ;
    skos:prefLabel "Item I293"@en-AU ;
    dcat:accessURL "https://www.legislation.gov.au/C2004A04997/2024-07-01/2024-07-01/text/1/epub/OEBPS/document_4/document_4.html#_Toc171752024"^^xsd:anyURI .

C2004A04997:294 a legcons:Chapter,
        skos:Concept,
        dcat:Resource ;
    rdfs:label "Chapter C294"@en-AU ;
    rdfs:comment "Chapter 70 Glass and glassware - GraphNodeID: C294"@en-AU ;
    skos:definition "Chapter 70 Glass and glassware"@en-AU ;
    skos:narrower C2004A04997:259 ;
    skos:prefLabel "Chapter C294"@en-AU ;
    dcat:accessURL "https://www.legislation.gov.au/C2004A04997/2024-07-01/2024-07-01/text/1/epub/OEBPS/document_4/document_4.html#_Toc171752025"^^xsd:anyURI .

C2004A04997:295 a legcons:Item,
        skos:Concept,
        dcat:Resource ;
    rdfs:label "Item I295"@en-AU ;
    rdfs:comment "Notes - GraphNodeID: I295"@en-AU ;
    skos:definition "Notes"@en-AU ;
    skos:narrower C2004A04997:56 ;
    skos:prefLabel "Item I295"@en-AU ;
    dcat:accessURL "https://www.legislation.gov.au/C2004A04997/2024-07-01/2024-07-01/text/1/epub/OEBPS/document_4/document_4.html#_Toc171752026"^^xsd:anyURI .

C2004A04997:296 a legcons:Item,
        skos:Concept,
        dcat:Resource ;
    rdfs:label "Item I296"@en-AU ;
    rdfs:comment "Subheading Note - GraphNodeID: I296"@en-AU ;
    skos:definition "Subheading Note"@en-AU ;
    skos:narrower C2004A04997:56 ;
    skos:prefLabel "Item I296"@en-AU ;
    dcat:accessURL "https://www.legislation.gov.au/C2004A04997/2024-07-01/2024-07-01/text/1/epub/OEBPS/document_4/document_4.html#_Toc171752027"^^xsd:anyURI .

C2004A04997:297 a legcons:Item,
        skos:Concept,
        dcat:Resource ;
    rdfs:label "Item I297"@en-AU ;
    rdfs:comment "Section XIVNatural or cultured pearls precious or semi precious stones precious metals metals clad with precious metal and articles thereof imitation jewellery coin - GraphNodeID: I297"@en-AU ;
    skos:definition "Section XIVNatural or cultured pearls precious or semi precious stones precious metals metals clad with precious metal and articles thereof imitation jewellery coin"@en-AU ;
    skos:narrower C2004A04997:56 ;
    skos:prefLabel "Item I297"@en-AU ;
    dcat:accessURL "https://www.legislation.gov.au/C2004A04997/2024-07-01/2024-07-01/text/1/epub/OEBPS/document_4/document_4.html#_Toc171752028"^^xsd:anyURI .

C2004A04997:298 a legcons:Chapter,
        skos:Concept,
        dcat:Resource ;
    rdfs:label "Chapter C298"@en-AU ;
    rdfs:comment "Chapter 71 Natural or cultured pearls precious or semi precious stones precious metals metals clad with precious metal and articles thereof imitation jewellery coin - GraphNodeID: C298"@en-AU ;
    skos:definition "Chapter 71 Natural or cultured pearls precious or semi precious stones precious metals metals clad with precious metal and articles thereof imitation jewellery coin"@en-AU ;
    skos:narrower C2004A04997:259 ;
    skos:prefLabel "Chapter C298"@en-AU ;
    dcat:accessURL "https://www.legislation.gov.au/C2004A04997/2024-07-01/2024-07-01/text/1/epub/OEBPS/document_4/document_4.html#_Toc171752029"^^xsd:anyURI .

C2004A04997:299 a legcons:Item,
        skos:Concept,
        dcat:Resource ;
    rdfs:label "Item I299"@en-AU ;
    rdfs:comment "Notes - GraphNodeID: I299"@en-AU ;
    skos:definition "Notes"@en-AU ;
    skos:narrower C2004A04997:56 ;
    skos:prefLabel "Item I299"@en-AU ;
    dcat:accessURL "https://www.legislation.gov.au/C2004A04997/2024-07-01/2024-07-01/text/1/epub/OEBPS/document_4/document_4.html#_Toc171752030"^^xsd:anyURI .

C2004A04997:3 a legcons:Item,
        skos:Concept,
        dcat:Resource ;
    rdfs:label "Item I3"@en-AU ;
    rdfs:comment "1  Short title - GraphNodeID: I3"@en-AU ;
    skos:definition "1  Short title"@en-AU ;
    skos:narrower C2004A04997:2 ;
    skos:prefLabel "Item I3"@en-AU ;
    dcat:accessURL "https://www.legislation.gov.au/C2004A04997/2024-07-01/2024-07-01/text/1/epub/OEBPS/document_1/document_1.html#_Toc172806503"^^xsd:anyURI .

C2004A04997:30 a legcons:Item,
        skos:Concept,
        dcat:Resource ;
    rdfs:label "Item I30"@en-AU ;
    rdfs:comment "13 H  When goods are Japanese originating goods - GraphNodeID: I30"@en-AU ;
    skos:definition "13 H  When goods are Japanese originating goods"@en-AU ;
    skos:narrower C2004A04997:2 ;
    skos:prefLabel "Item I30"@en-AU ;
    dcat:accessURL "https://www.legislation.gov.au/C2004A04997/2024-07-01/2024-07-01/text/1/epub/OEBPS/document_1/document_1.html#_Toc172806530"^^xsd:anyURI .

C2004A04997:300 a legcons:Item,
        skos:Concept,
        dcat:Resource ;
    rdfs:label "Item I300"@en-AU ;
    rdfs:comment "Subheading Notes - GraphNodeID: I300"@en-AU ;
    skos:definition "Subheading Notes"@en-AU ;
    skos:narrower C2004A04997:56 ;
    skos:prefLabel "Item I300"@en-AU ;
    dcat:accessURL "https://www.legislation.gov.au/C2004A04997/2024-07-01/2024-07-01/text/1/epub/OEBPS/document_4/document_4.html#_Toc171752031"^^xsd:anyURI .

C2004A04997:301 a legcons:Item,
        skos:Concept,
        dcat:Resource ;
    rdfs:label "Item I301"@en-AU ;
    rdfs:comment "Sub Chapter INatural or cultured pearls and precious or semi precious stones - GraphNodeID: I301"@en-AU ;
    skos:definition "Sub Chapter INatural or cultured pearls and precious or semi precious stones"@en-AU ;
    skos:narrower C2004A04997:56 ;
    skos:prefLabel "Item I301"@en-AU ;
    dcat:accessURL "https://www.legislation.gov.au/C2004A04997/2024-07-01/2024-07-01/text/1/epub/OEBPS/document_4/document_4.html#_Toc171752032"^^xsd:anyURI .

C2004A04997:302 a legcons:Item,
        skos:Concept,
        dcat:Resource ;
    rdfs:label "Item I302"@en-AU ;
    rdfs:comment "Sub Chapter IIPrecious metals and metals clad with precious metal - GraphNodeID: I302"@en-AU ;
    skos:definition "Sub Chapter IIPrecious metals and metals clad with precious metal"@en-AU ;
    skos:narrower C2004A04997:56 ;
    skos:prefLabel "Item I302"@en-AU ;
    dcat:accessURL "https://www.legislation.gov.au/C2004A04997/2024-07-01/2024-07-01/text/1/epub/OEBPS/document_4/document_4.html#_Toc171752033"^^xsd:anyURI .

C2004A04997:303 a legcons:Item,
        skos:Concept,
        dcat:Resource ;
    rdfs:label "Item I303"@en-AU ;
    rdfs:comment "Sub Chapter IIIJewellery goldsmiths and silversmiths wares and other articles - GraphNodeID: I303"@en-AU ;
    skos:definition "Sub Chapter IIIJewellery goldsmiths and silversmiths wares and other articles"@en-AU ;
    skos:narrower C2004A04997:56 ;
    skos:prefLabel "Item I303"@en-AU ;
    dcat:accessURL "https://www.legislation.gov.au/C2004A04997/2024-07-01/2024-07-01/text/1/epub/OEBPS/document_4/document_4.html#_Toc171752034"^^xsd:anyURI .

C2004A04997:304 a legcons:Item,
        skos:Concept,
        dcat:Resource ;
    rdfs:label "Item I304"@en-AU ;
    rdfs:comment "Section XVBase metals and articles of base metal - GraphNodeID: I304"@en-AU ;
    skos:definition "Section XVBase metals and articles of base metal"@en-AU ;
    skos:narrower C2004A04997:56 ;
    skos:prefLabel "Item I304"@en-AU ;
    dcat:accessURL "https://www.legislation.gov.au/C2004A04997/2024-07-01/2024-07-01/text/1/epub/OEBPS/document_4/document_4.html#_Toc171752035"^^xsd:anyURI .

C2004A04997:305 a legcons:Item,
        skos:Concept,
        dcat:Resource ;
    rdfs:label "Item I305"@en-AU ;
    rdfs:comment "Notes - GraphNodeID: I305"@en-AU ;
    skos:definition "Notes"@en-AU ;
    skos:narrower C2004A04997:56 ;
    skos:prefLabel "Item I305"@en-AU ;
    dcat:accessURL "https://www.legislation.gov.au/C2004A04997/2024-07-01/2024-07-01/text/1/epub/OEBPS/document_4/document_4.html#_Toc171752036"^^xsd:anyURI .

C2004A04997:306 a legcons:Chapter,
        skos:Concept,
        dcat:Resource ;
    rdfs:label "Chapter C306"@en-AU ;
    rdfs:comment "Chapter 72 Iron and steel - GraphNodeID: C306"@en-AU ;
    skos:definition "Chapter 72 Iron and steel"@en-AU ;
    skos:narrower C2004A04997:259 ;
    skos:prefLabel "Chapter C306"@en-AU ;
    dcat:accessURL "https://www.legislation.gov.au/C2004A04997/2024-07-01/2024-07-01/text/1/epub/OEBPS/document_4/document_4.html#_Toc171752037"^^xsd:anyURI .

C2004A04997:307 a legcons:Item,
        skos:Concept,
        dcat:Resource ;
    rdfs:label "Item I307"@en-AU ;
    rdfs:comment "Notes - GraphNodeID: I307"@en-AU ;
    skos:definition "Notes"@en-AU ;
    skos:narrower C2004A04997:56 ;
    skos:prefLabel "Item I307"@en-AU ;
    dcat:accessURL "https://www.legislation.gov.au/C2004A04997/2024-07-01/2024-07-01/text/1/epub/OEBPS/document_4/document_4.html#_Toc171752038"^^xsd:anyURI .

C2004A04997:308 a legcons:Item,
        skos:Concept,
        dcat:Resource ;
    rdfs:label "Item I308"@en-AU ;
    rdfs:comment "Subheading Notes - GraphNodeID: I308"@en-AU ;
    skos:definition "Subheading Notes"@en-AU ;
    skos:narrower C2004A04997:56 ;
    skos:prefLabel "Item I308"@en-AU ;
    dcat:accessURL "https://www.legislation.gov.au/C2004A04997/2024-07-01/2024-07-01/text/1/epub/OEBPS/document_4/document_4.html#_Toc171752039"^^xsd:anyURI .

C2004A04997:309 a legcons:Item,
        skos:Concept,
        dcat:Resource ;
    rdfs:label "Item I309"@en-AU ;
    rdfs:comment "Additional Note - GraphNodeID: I309"@en-AU ;
    skos:definition "Additional Note"@en-AU ;
    skos:narrower C2004A04997:56 ;
    skos:prefLabel "Item I309"@en-AU ;
    dcat:accessURL "https://www.legislation.gov.au/C2004A04997/2024-07-01/2024-07-01/text/1/epub/OEBPS/document_4/document_4.html#_Toc171752040"^^xsd:anyURI .

C2004A04997:31 a legcons:Item,
        skos:Concept,
        dcat:Resource ;
    rdfs:label "Item I31"@en-AU ;
    rdfs:comment "13 J  When goods are Chinese originating goods - GraphNodeID: I31"@en-AU ;
    skos:definition "13 J  When goods are Chinese originating goods"@en-AU ;
    skos:narrower C2004A04997:2 ;
    skos:prefLabel "Item I31"@en-AU ;
    dcat:accessURL "https://www.legislation.gov.au/C2004A04997/2024-07-01/2024-07-01/text/1/epub/OEBPS/document_1/document_1.html#_Toc172806531"^^xsd:anyURI .

C2004A04997:310 a legcons:Item,
        skos:Concept,
        dcat:Resource ;
    rdfs:label "Item I310"@en-AU ;
    rdfs:comment "Sub Chapter IPrimary materials products in granular or powder form - GraphNodeID: I310"@en-AU ;
    skos:definition "Sub Chapter IPrimary materials products in granular or powder form"@en-AU ;
    skos:narrower C2004A04997:56 ;
    skos:prefLabel "Item I310"@en-AU ;
    dcat:accessURL "https://www.legislation.gov.au/C2004A04997/2024-07-01/2024-07-01/text/1/epub/OEBPS/document_4/document_4.html#_Toc171752041"^^xsd:anyURI .

C2004A04997:311 a legcons:Item,
        skos:Concept,
        dcat:Resource ;
    rdfs:label "Item I311"@en-AU ;
    rdfs:comment "Sub Chapter IIIron and non alloy steel - GraphNodeID: I311"@en-AU ;
    skos:definition "Sub Chapter IIIron and non alloy steel"@en-AU ;
    skos:narrower C2004A04997:56 ;
    skos:prefLabel "Item I311"@en-AU ;
    dcat:accessURL "https://www.legislation.gov.au/C2004A04997/2024-07-01/2024-07-01/text/1/epub/OEBPS/document_4/document_4.html#_Toc171752042"^^xsd:anyURI .

C2004A04997:312 a legcons:Item,
        skos:Concept,
        dcat:Resource ;
    rdfs:label "Item I312"@en-AU ;
    rdfs:comment "Sub Chapter IIIStainless steel - GraphNodeID: I312"@en-AU ;
    skos:definition "Sub Chapter IIIStainless steel"@en-AU ;
    skos:narrower C2004A04997:56 ;
    skos:prefLabel "Item I312"@en-AU ;
    dcat:accessURL "https://www.legislation.gov.au/C2004A04997/2024-07-01/2024-07-01/text/1/epub/OEBPS/document_4/document_4.html#_Toc171752043"^^xsd:anyURI .

C2004A04997:313 a legcons:Item,
        skos:Concept,
        dcat:Resource ;
    rdfs:label "Item I313"@en-AU ;
    rdfs:comment "Sub Chapter IVOther alloy steel hollow drill bars and rods of alloy or non alloy steel - GraphNodeID: I313"@en-AU ;
    skos:definition "Sub Chapter IVOther alloy steel hollow drill bars and rods of alloy or non alloy steel"@en-AU ;
    skos:narrower C2004A04997:56 ;
    skos:prefLabel "Item I313"@en-AU ;
    dcat:accessURL "https://www.legislation.gov.au/C2004A04997/2024-07-01/2024-07-01/text/1/epub/OEBPS/document_4/document_4.html#_Toc171752044"^^xsd:anyURI .

C2004A04997:314 a legcons:Chapter,
        skos:Concept,
        dcat:Resource ;
    rdfs:label "Chapter C314"@en-AU ;
    rdfs:comment "Chapter 73 Articles of iron or steel - GraphNodeID: C314"@en-AU ;
    skos:definition "Chapter 73 Articles of iron or steel"@en-AU ;
    skos:narrower C2004A04997:259 ;
    skos:prefLabel "Chapter C314"@en-AU ;
    dcat:accessURL "https://www.legislation.gov.au/C2004A04997/2024-07-01/2024-07-01/text/1/epub/OEBPS/document_4/document_4.html#_Toc171752045"^^xsd:anyURI .

C2004A04997:315 a legcons:Item,
        skos:Concept,
        dcat:Resource ;
    rdfs:label "Item I315"@en-AU ;
    rdfs:comment "Notes - GraphNodeID: I315"@en-AU ;
    skos:definition "Notes"@en-AU ;
    skos:narrower C2004A04997:56 ;
    skos:prefLabel "Item I315"@en-AU ;
    dcat:accessURL "https://www.legislation.gov.au/C2004A04997/2024-07-01/2024-07-01/text/1/epub/OEBPS/document_4/document_4.html#_Toc171752046"^^xsd:anyURI .

C2004A04997:316 a legcons:Item,
        skos:Concept,
        dcat:Resource ;
    rdfs:label "Item I316"@en-AU ;
    rdfs:comment "Additional Notes - GraphNodeID: I316"@en-AU ;
    skos:definition "Additional Notes"@en-AU ;
    skos:narrower C2004A04997:56 ;
    skos:prefLabel "Item I316"@en-AU ;
    dcat:accessURL "https://www.legislation.gov.au/C2004A04997/2024-07-01/2024-07-01/text/1/epub/OEBPS/document_4/document_4.html#_Toc171752047"^^xsd:anyURI .

C2004A04997:318 a legcons:Item,
        skos:Concept,
        dcat:Resource ;
    rdfs:label "Item I318"@en-AU ;
    rdfs:comment "Schedule 3 Classification of goods and general and special rates of duty - GraphNodeID: I318"@en-AU ;
    skos:definition "Schedule 3 Classification of goods and general and special rates of duty"@en-AU ;
    skos:narrower C2004A04997:56 ;
    skos:prefLabel "Item I318"@en-AU ;
    dcat:accessURL "https://www.legislation.gov.au/C2004A04997/2024-07-01/2024-07-01/text/1/epub/OEBPS/document_5/document_5.html#_Toc171753160"^^xsd:anyURI .

C2004A04997:319 a legcons:Item,
        skos:Concept,
        dcat:Resource ;
    rdfs:label "Item I319"@en-AU ;
    rdfs:comment "Section XVBase metals and articles of base metal - GraphNodeID: I319"@en-AU ;
    skos:definition "Section XVBase metals and articles of base metal"@en-AU ;
    skos:narrower C2004A04997:56 ;
    skos:prefLabel "Item I319"@en-AU ;
    dcat:accessURL "https://www.legislation.gov.au/C2004A04997/2024-07-01/2024-07-01/text/1/epub/OEBPS/document_5/document_5.html#_Toc171753161"^^xsd:anyURI .

C2004A04997:32 a legcons:Item,
        skos:Concept,
        dcat:Resource ;
    rdfs:label "Item I32"@en-AU ;
    rdfs:comment "13 K  When goods are Hong Kong originating goods - GraphNodeID: I32"@en-AU ;
    skos:definition "13 K  When goods are Hong Kong originating goods"@en-AU ;
    skos:narrower C2004A04997:2 ;
    skos:prefLabel "Item I32"@en-AU ;
    dcat:accessURL "https://www.legislation.gov.au/C2004A04997/2024-07-01/2024-07-01/text/1/epub/OEBPS/document_1/document_1.html#_Toc172806532"^^xsd:anyURI .

C2004A04997:320 a legcons:Chapter,
        skos:Concept,
        dcat:Resource ;
    rdfs:label "Chapter C320"@en-AU ;
    rdfs:comment "Chapter 74 Copper and articles thereof - GraphNodeID: C320"@en-AU ;
    skos:definition "Chapter 74 Copper and articles thereof"@en-AU ;
    skos:narrower C2004A04997:317 ;
    skos:prefLabel "Chapter C320"@en-AU ;
    dcat:accessURL "https://www.legislation.gov.au/C2004A04997/2024-07-01/2024-07-01/text/1/epub/OEBPS/document_5/document_5.html#_Toc171753162"^^xsd:anyURI .

C2004A04997:321 a legcons:Item,
        skos:Concept,
        dcat:Resource ;
    rdfs:label "Item I321"@en-AU ;
    rdfs:comment "Note - GraphNodeID: I321"@en-AU ;
    skos:definition "Note"@en-AU ;
    skos:narrower C2004A04997:56 ;
    skos:prefLabel "Item I321"@en-AU ;
    dcat:accessURL "https://www.legislation.gov.au/C2004A04997/2024-07-01/2024-07-01/text/1/epub/OEBPS/document_5/document_5.html#_Toc171753163"^^xsd:anyURI .

C2004A04997:322 a legcons:Item,
        skos:Concept,
        dcat:Resource ;
    rdfs:label "Item I322"@en-AU ;
    rdfs:comment "Subheading Note - GraphNodeID: I322"@en-AU ;
    skos:definition "Subheading Note"@en-AU ;
    skos:narrower C2004A04997:56 ;
    skos:prefLabel "Item I322"@en-AU ;
    dcat:accessURL "https://www.legislation.gov.au/C2004A04997/2024-07-01/2024-07-01/text/1/epub/OEBPS/document_5/document_5.html#_Toc171753164"^^xsd:anyURI .

C2004A04997:323 a legcons:Chapter,
        skos:Concept,
        dcat:Resource ;
    rdfs:label "Chapter C323"@en-AU ;
    rdfs:comment "Chapter 75 Nickel and articles thereof - GraphNodeID: C323"@en-AU ;
    skos:definition "Chapter 75 Nickel and articles thereof"@en-AU ;
    skos:narrower C2004A04997:317 ;
    skos:prefLabel "Chapter C323"@en-AU ;
    dcat:accessURL "https://www.legislation.gov.au/C2004A04997/2024-07-01/2024-07-01/text/1/epub/OEBPS/document_5/document_5.html#_Toc171753165"^^xsd:anyURI .

C2004A04997:324 a legcons:Item,
        skos:Concept,
        dcat:Resource ;
    rdfs:label "Item I324"@en-AU ;
    rdfs:comment "Subheading Notes - GraphNodeID: I324"@en-AU ;
    skos:definition "Subheading Notes"@en-AU ;
    skos:narrower C2004A04997:56 ;
    skos:prefLabel "Item I324"@en-AU ;
    dcat:accessURL "https://www.legislation.gov.au/C2004A04997/2024-07-01/2024-07-01/text/1/epub/OEBPS/document_5/document_5.html#_Toc171753166"^^xsd:anyURI .

C2004A04997:325 a legcons:Chapter,
        skos:Concept,
        dcat:Resource ;
    rdfs:label "Chapter C325"@en-AU ;
    rdfs:comment "Chapter 76 Aluminium and articles thereof - GraphNodeID: C325"@en-AU ;
    skos:definition "Chapter 76 Aluminium and articles thereof"@en-AU ;
    skos:narrower C2004A04997:317 ;
    skos:prefLabel "Chapter C325"@en-AU ;
    dcat:accessURL "https://www.legislation.gov.au/C2004A04997/2024-07-01/2024-07-01/text/1/epub/OEBPS/document_5/document_5.html#_Toc171753167"^^xsd:anyURI .

C2004A04997:326 a legcons:Item,
        skos:Concept,
        dcat:Resource ;
    rdfs:label "Item I326"@en-AU ;
    rdfs:comment "Subheading Notes - GraphNodeID: I326"@en-AU ;
    skos:definition "Subheading Notes"@en-AU ;
    skos:narrower C2004A04997:56 ;
    skos:prefLabel "Item I326"@en-AU ;
    dcat:accessURL "https://www.legislation.gov.au/C2004A04997/2024-07-01/2024-07-01/text/1/epub/OEBPS/document_5/document_5.html#_Toc171753168"^^xsd:anyURI .

C2004A04997:327 a legcons:Item,
        skos:Concept,
        dcat:Resource ;
    rdfs:label "Item I327"@en-AU ;
    rdfs:comment "Additional Note - GraphNodeID: I327"@en-AU ;
    skos:definition "Additional Note"@en-AU ;
    skos:narrower C2004A04997:56 ;
    skos:prefLabel "Item I327"@en-AU ;
    dcat:accessURL "https://www.legislation.gov.au/C2004A04997/2024-07-01/2024-07-01/text/1/epub/OEBPS/document_5/document_5.html#_Toc171753169"^^xsd:anyURI .

C2004A04997:328 a legcons:Chapter,
        skos:Concept,
        dcat:Resource ;
    rdfs:label "Chapter C328"@en-AU ;
    rdfs:comment "Chapter 78 Lead and articles thereof - GraphNodeID: C328"@en-AU ;
    skos:definition "Chapter 78 Lead and articles thereof"@en-AU ;
    skos:narrower C2004A04997:317 ;
    skos:prefLabel "Chapter C328"@en-AU ;
    dcat:accessURL "https://www.legislation.gov.au/C2004A04997/2024-07-01/2024-07-01/text/1/epub/OEBPS/document_5/document_5.html#_Toc171753170"^^xsd:anyURI .

C2004A04997:329 a legcons:Item,
        skos:Concept,
        dcat:Resource ;
    rdfs:label "Item I329"@en-AU ;
    rdfs:comment "Subheading Note - GraphNodeID: I329"@en-AU ;
    skos:definition "Subheading Note"@en-AU ;
    skos:narrower C2004A04997:56 ;
    skos:prefLabel "Item I329"@en-AU ;
    dcat:accessURL "https://www.legislation.gov.au/C2004A04997/2024-07-01/2024-07-01/text/1/epub/OEBPS/document_5/document_5.html#_Toc171753171"^^xsd:anyURI .

C2004A04997:33 a legcons:Item,
        skos:Concept,
        dcat:Resource ;
    rdfs:label "Item I33"@en-AU ;
    rdfs:comment "13 L  When goods are Regional Comprehensive Economic Partnership RCEP originating goods - GraphNodeID: I33"@en-AU ;
    skos:definition "13 L  When goods are Regional Comprehensive Economic Partnership RCEP originating goods"@en-AU ;
    skos:narrower C2004A04997:2 ;
    skos:prefLabel "Item I33"@en-AU ;
    dcat:accessURL "https://www.legislation.gov.au/C2004A04997/2024-07-01/2024-07-01/text/1/epub/OEBPS/document_1/document_1.html#_Toc172806533"^^xsd:anyURI .

C2004A04997:330 a legcons:Chapter,
        skos:Concept,
        dcat:Resource ;
    rdfs:label "Chapter C330"@en-AU ;
    rdfs:comment "Chapter 79 Zinc and articles thereof - GraphNodeID: C330"@en-AU ;
    skos:definition "Chapter 79 Zinc and articles thereof"@en-AU ;
    skos:narrower C2004A04997:317 ;
    skos:prefLabel "Chapter C330"@en-AU ;
    dcat:accessURL "https://www.legislation.gov.au/C2004A04997/2024-07-01/2024-07-01/text/1/epub/OEBPS/document_5/document_5.html#_Toc171753172"^^xsd:anyURI .

C2004A04997:331 a legcons:Item,
        skos:Concept,
        dcat:Resource ;
    rdfs:label "Item I331"@en-AU ;
    rdfs:comment "Subheading Note - GraphNodeID: I331"@en-AU ;
    skos:definition "Subheading Note"@en-AU ;
    skos:narrower C2004A04997:56 ;
    skos:prefLabel "Item I331"@en-AU ;
    dcat:accessURL "https://www.legislation.gov.au/C2004A04997/2024-07-01/2024-07-01/text/1/epub/OEBPS/document_5/document_5.html#_Toc171753173"^^xsd:anyURI .

C2004A04997:332 a legcons:Chapter,
        skos:Concept,
        dcat:Resource ;
    rdfs:label "Chapter C332"@en-AU ;
    rdfs:comment "Chapter 80 Tin and articles thereof - GraphNodeID: C332"@en-AU ;
    skos:definition "Chapter 80 Tin and articles thereof"@en-AU ;
    skos:narrower C2004A04997:317 ;
    skos:prefLabel "Chapter C332"@en-AU ;
    dcat:accessURL "https://www.legislation.gov.au/C2004A04997/2024-07-01/2024-07-01/text/1/epub/OEBPS/document_5/document_5.html#_Toc171753174"^^xsd:anyURI .

C2004A04997:333 a legcons:Item,
        skos:Concept,
        dcat:Resource ;
    rdfs:label "Item I333"@en-AU ;
    rdfs:comment "Subheading Note - GraphNodeID: I333"@en-AU ;
    skos:definition "Subheading Note"@en-AU ;
    skos:narrower C2004A04997:56 ;
    skos:prefLabel "Item I333"@en-AU ;
    dcat:accessURL "https://www.legislation.gov.au/C2004A04997/2024-07-01/2024-07-01/text/1/epub/OEBPS/document_5/document_5.html#_Toc171753175"^^xsd:anyURI .

C2004A04997:334 a legcons:Chapter,
        skos:Concept,
        dcat:Resource ;
    rdfs:label "Chapter C334"@en-AU ;
    rdfs:comment "Chapter 81 Other base metals cermets articles thereof - GraphNodeID: C334"@en-AU ;
    skos:definition "Chapter 81 Other base metals cermets articles thereof"@en-AU ;
    skos:narrower C2004A04997:317 ;
    skos:prefLabel "Chapter C334"@en-AU ;
    dcat:accessURL "https://www.legislation.gov.au/C2004A04997/2024-07-01/2024-07-01/text/1/epub/OEBPS/document_5/document_5.html#_Toc171753176"^^xsd:anyURI .

C2004A04997:335 a legcons:Chapter,
        skos:Concept,
        dcat:Resource ;
    rdfs:label "Chapter C335"@en-AU ;
    rdfs:comment "Chapter 82 Tools implements cutlery spoons and forks of base metal parts thereof of base metal - GraphNodeID: C335"@en-AU ;
    skos:definition "Chapter 82 Tools implements cutlery spoons and forks of base metal parts thereof of base metal"@en-AU ;
    skos:narrower C2004A04997:317 ;
    skos:prefLabel "Chapter C335"@en-AU ;
    dcat:accessURL "https://www.legislation.gov.au/C2004A04997/2024-07-01/2024-07-01/text/1/epub/OEBPS/document_5/document_5.html#_Toc171753177"^^xsd:anyURI .

C2004A04997:336 a legcons:Item,
        skos:Concept,
        dcat:Resource ;
    rdfs:label "Item I336"@en-AU ;
    rdfs:comment "Notes - GraphNodeID: I336"@en-AU ;
    skos:definition "Notes"@en-AU ;
    skos:narrower C2004A04997:56 ;
    skos:prefLabel "Item I336"@en-AU ;
    dcat:accessURL "https://www.legislation.gov.au/C2004A04997/2024-07-01/2024-07-01/text/1/epub/OEBPS/document_5/document_5.html#_Toc171753178"^^xsd:anyURI .

C2004A04997:337 a legcons:Chapter,
        skos:Concept,
        dcat:Resource ;
    rdfs:label "Chapter C337"@en-AU ;
    rdfs:comment "Chapter 83 Miscellaneous articles of base metal - GraphNodeID: C337"@en-AU ;
    skos:definition "Chapter 83 Miscellaneous articles of base metal"@en-AU ;
    skos:narrower C2004A04997:317 ;
    skos:prefLabel "Chapter C337"@en-AU ;
    dcat:accessURL "https://www.legislation.gov.au/C2004A04997/2024-07-01/2024-07-01/text/1/epub/OEBPS/document_5/document_5.html#_Toc171753179"^^xsd:anyURI .

C2004A04997:338 a legcons:Item,
        skos:Concept,
        dcat:Resource ;
    rdfs:label "Item I338"@en-AU ;
    rdfs:comment "Notes - GraphNodeID: I338"@en-AU ;
    skos:definition "Notes"@en-AU ;
    skos:narrower C2004A04997:56 ;
    skos:prefLabel "Item I338"@en-AU ;
    dcat:accessURL "https://www.legislation.gov.au/C2004A04997/2024-07-01/2024-07-01/text/1/epub/OEBPS/document_5/document_5.html#_Toc171753180"^^xsd:anyURI .

C2004A04997:339 a legcons:Item,
        skos:Concept,
        dcat:Resource ;
    rdfs:label "Item I339"@en-AU ;
    rdfs:comment "Additional Note - GraphNodeID: I339"@en-AU ;
    skos:definition "Additional Note"@en-AU ;
    skos:narrower C2004A04997:56 ;
    skos:prefLabel "Item I339"@en-AU ;
    dcat:accessURL "https://www.legislation.gov.au/C2004A04997/2024-07-01/2024-07-01/text/1/epub/OEBPS/document_5/document_5.html#_Toc171753181"^^xsd:anyURI .

C2004A04997:34 a legcons:Item,
        skos:Concept,
        dcat:Resource ;
    rdfs:label "Item I34"@en-AU ;
    rdfs:comment "13 M  When goods are UK originating goods - GraphNodeID: I34"@en-AU ;
    skos:definition "13 M  When goods are UK originating goods"@en-AU ;
    skos:narrower C2004A04997:2 ;
    skos:prefLabel "Item I34"@en-AU ;
    dcat:accessURL "https://www.legislation.gov.au/C2004A04997/2024-07-01/2024-07-01/text/1/epub/OEBPS/document_1/document_1.html#_Toc172806534"^^xsd:anyURI .

C2004A04997:340 a legcons:Item,
        skos:Concept,
        dcat:Resource ;
    rdfs:label "Item I340"@en-AU ;
    rdfs:comment "Section XVIMachinery and mechanical appliances electrical equipment parts thereof sound recorders and reproducers television image and sound recorders and reproducers and parts and accessories of such articles - GraphNodeID: I340"@en-AU ;
    skos:definition "Section XVIMachinery and mechanical appliances electrical equipment parts thereof sound recorders and reproducers television image and sound recorders and reproducers and parts and accessories of such articles"@en-AU ;
    skos:narrower C2004A04997:56 ;
    skos:prefLabel "Item I340"@en-AU ;
    dcat:accessURL "https://www.legislation.gov.au/C2004A04997/2024-07-01/2024-07-01/text/1/epub/OEBPS/document_5/document_5.html#_Toc171753182"^^xsd:anyURI .

C2004A04997:341 a legcons:Item,
        skos:Concept,
        dcat:Resource ;
    rdfs:label "Item I341"@en-AU ;
    rdfs:comment "Notes - GraphNodeID: I341"@en-AU ;
    skos:definition "Notes"@en-AU ;
    skos:narrower C2004A04997:56 ;
    skos:prefLabel "Item I341"@en-AU ;
    dcat:accessURL "https://www.legislation.gov.au/C2004A04997/2024-07-01/2024-07-01/text/1/epub/OEBPS/document_5/document_5.html#_Toc171753183"^^xsd:anyURI .

C2004A04997:342 a legcons:Item,
        skos:Concept,
        dcat:Resource ;
    rdfs:label "Item I342"@en-AU ;
    rdfs:comment "Additional Notes - GraphNodeID: I342"@en-AU ;
    skos:definition "Additional Notes"@en-AU ;
    skos:narrower C2004A04997:56 ;
    skos:prefLabel "Item I342"@en-AU ;
    dcat:accessURL "https://www.legislation.gov.au/C2004A04997/2024-07-01/2024-07-01/text/1/epub/OEBPS/document_5/document_5.html#_Toc171753184"^^xsd:anyURI .

C2004A04997:343 a legcons:Chapter,
        skos:Concept,
        dcat:Resource ;
    rdfs:label "Chapter C343"@en-AU ;
    rdfs:comment "Chapter 84 Nuclear reactors boilers machinery and mechanical appliances parts thereof - GraphNodeID: C343"@en-AU ;
    skos:definition "Chapter 84 Nuclear reactors boilers machinery and mechanical appliances parts thereof"@en-AU ;
    skos:narrower C2004A04997:317 ;
    skos:prefLabel "Chapter C343"@en-AU ;
    dcat:accessURL "https://www.legislation.gov.au/C2004A04997/2024-07-01/2024-07-01/text/1/epub/OEBPS/document_5/document_5.html#_Toc171753185"^^xsd:anyURI .

C2004A04997:344 a legcons:Item,
        skos:Concept,
        dcat:Resource ;
    rdfs:label "Item I344"@en-AU ;
    rdfs:comment "Notes - GraphNodeID: I344"@en-AU ;
    skos:definition "Notes"@en-AU ;
    skos:narrower C2004A04997:56 ;
    skos:prefLabel "Item I344"@en-AU ;
    dcat:accessURL "https://www.legislation.gov.au/C2004A04997/2024-07-01/2024-07-01/text/1/epub/OEBPS/document_5/document_5.html#_Toc171753186"^^xsd:anyURI .

C2004A04997:345 a legcons:Item,
        skos:Concept,
        dcat:Resource ;
    rdfs:label "Item I345"@en-AU ;
    rdfs:comment "Subheading Notes - GraphNodeID: I345"@en-AU ;
    skos:definition "Subheading Notes"@en-AU ;
    skos:narrower C2004A04997:56 ;
    skos:prefLabel "Item I345"@en-AU ;
    dcat:accessURL "https://www.legislation.gov.au/C2004A04997/2024-07-01/2024-07-01/text/1/epub/OEBPS/document_5/document_5.html#_Toc171753187"^^xsd:anyURI .

C2004A04997:346 a legcons:Item,
        skos:Concept,
        dcat:Resource ;
    rdfs:label "Item I346"@en-AU ;
    rdfs:comment "Additional Notes - GraphNodeID: I346"@en-AU ;
    skos:definition "Additional Notes"@en-AU ;
    skos:narrower C2004A04997:56 ;
    skos:prefLabel "Item I346"@en-AU ;
    dcat:accessURL "https://www.legislation.gov.au/C2004A04997/2024-07-01/2024-07-01/text/1/epub/OEBPS/document_5/document_5.html#_Toc171753188"^^xsd:anyURI .

C2004A04997:347 a legcons:Chapter,
        skos:Concept,
        dcat:Resource ;
    rdfs:label "Chapter C347"@en-AU ;
    rdfs:comment "Chapter 85 Electrical machinery and equipment and parts thereof sound recorders and reproducers television image and sound recorders and reproducers and parts and accessories of such articles - GraphNodeID: C347"@en-AU ;
    skos:definition "Chapter 85 Electrical machinery and equipment and parts thereof sound recorders and reproducers television image and sound recorders and reproducers and parts and accessories of such articles"@en-AU ;
    skos:narrower C2004A04997:317 ;
    skos:prefLabel "Chapter C347"@en-AU ;
    dcat:accessURL "https://www.legislation.gov.au/C2004A04997/2024-07-01/2024-07-01/text/1/epub/OEBPS/document_5/document_5.html#_Toc171753189"^^xsd:anyURI .

C2004A04997:348 a legcons:Item,
        skos:Concept,
        dcat:Resource ;
    rdfs:label "Item I348"@en-AU ;
    rdfs:comment "Notes - GraphNodeID: I348"@en-AU ;
    skos:definition "Notes"@en-AU ;
    skos:narrower C2004A04997:56 ;
    skos:prefLabel "Item I348"@en-AU ;
    dcat:accessURL "https://www.legislation.gov.au/C2004A04997/2024-07-01/2024-07-01/text/1/epub/OEBPS/document_5/document_5.html#_Toc171753190"^^xsd:anyURI .

C2004A04997:349 a legcons:Item,
        skos:Concept,
        dcat:Resource ;
    rdfs:label "Item I349"@en-AU ;
    rdfs:comment "Subheading Notes - GraphNodeID: I349"@en-AU ;
    skos:definition "Subheading Notes"@en-AU ;
    skos:narrower C2004A04997:56 ;
    skos:prefLabel "Item I349"@en-AU ;
    dcat:accessURL "https://www.legislation.gov.au/C2004A04997/2024-07-01/2024-07-01/text/1/epub/OEBPS/document_5/document_5.html#_Toc171753191"^^xsd:anyURI .

C2004A04997:35 a legcons:Item,
        skos:Concept,
        dcat:Resource ;
    rdfs:label "Item I35"@en-AU ;
    rdfs:comment "14  Application of rates of duty in relation to countries and places - GraphNodeID: I35"@en-AU ;
    skos:definition "14  Application of rates of duty in relation to countries and places"@en-AU ;
    skos:narrower C2004A04997:2 ;
    skos:prefLabel "Item I35"@en-AU ;
    dcat:accessURL "https://www.legislation.gov.au/C2004A04997/2024-07-01/2024-07-01/text/1/epub/OEBPS/document_1/document_1.html#_Toc172806535"^^xsd:anyURI .

C2004A04997:350 a legcons:Item,
        skos:Concept,
        dcat:Resource ;
    rdfs:label "Item I350"@en-AU ;
    rdfs:comment "Additional Notes - GraphNodeID: I350"@en-AU ;
    skos:definition "Additional Notes"@en-AU ;
    skos:narrower C2004A04997:56 ;
    skos:prefLabel "Item I350"@en-AU ;
    dcat:accessURL "https://www.legislation.gov.au/C2004A04997/2024-07-01/2024-07-01/text/1/epub/OEBPS/document_5/document_5.html#_Toc171753192"^^xsd:anyURI .

C2004A04997:351 a legcons:Item,
        skos:Concept,
        dcat:Resource ;
    rdfs:label "Item I351"@en-AU ;
    rdfs:comment "Section XVIIVehicles aircraft vessels and associated transport equipment - GraphNodeID: I351"@en-AU ;
    skos:definition "Section XVIIVehicles aircraft vessels and associated transport equipment"@en-AU ;
    skos:narrower C2004A04997:56 ;
    skos:prefLabel "Item I351"@en-AU ;
    dcat:accessURL "https://www.legislation.gov.au/C2004A04997/2024-07-01/2024-07-01/text/1/epub/OEBPS/document_5/document_5.html#_Toc171753193"^^xsd:anyURI .

C2004A04997:352 a legcons:Item,
        skos:Concept,
        dcat:Resource ;
    rdfs:label "Item I352"@en-AU ;
    rdfs:comment "Notes - GraphNodeID: I352"@en-AU ;
    skos:definition "Notes"@en-AU ;
    skos:narrower C2004A04997:56 ;
    skos:prefLabel "Item I352"@en-AU ;
    dcat:accessURL "https://www.legislation.gov.au/C2004A04997/2024-07-01/2024-07-01/text/1/epub/OEBPS/document_5/document_5.html#_Toc171753194"^^xsd:anyURI .

C2004A04997:353 a legcons:Chapter,
        skos:Concept,
        dcat:Resource ;
    rdfs:label "Chapter C353"@en-AU ;
    rdfs:comment "Chapter 86 Railway or tramway locomotives rolling stock and parts thereof railway or tramway track fixtures and fittings and parts thereof mechanical including electro mechanical traffic signalling equipment of all kinds - GraphNodeID: C353"@en-AU ;
    skos:definition "Chapter 86 Railway or tramway locomotives rolling stock and parts thereof railway or tramway track fixtures and fittings and parts thereof mechanical including electro mechanical traffic signalling equipment of all kinds"@en-AU ;
    skos:narrower C2004A04997:317 ;
    skos:prefLabel "Chapter C353"@en-AU ;
    dcat:accessURL "https://www.legislation.gov.au/C2004A04997/2024-07-01/2024-07-01/text/1/epub/OEBPS/document_5/document_5.html#_Toc171753195"^^xsd:anyURI .

C2004A04997:354 a legcons:Item,
        skos:Concept,
        dcat:Resource ;
    rdfs:label "Item I354"@en-AU ;
    rdfs:comment "Notes - GraphNodeID: I354"@en-AU ;
    skos:definition "Notes"@en-AU ;
    skos:narrower C2004A04997:56 ;
    skos:prefLabel "Item I354"@en-AU ;
    dcat:accessURL "https://www.legislation.gov.au/C2004A04997/2024-07-01/2024-07-01/text/1/epub/OEBPS/document_5/document_5.html#_Toc171753196"^^xsd:anyURI .

C2004A04997:355 a legcons:Chapter,
        skos:Concept,
        dcat:Resource ;
    rdfs:label "Chapter C355"@en-AU ;
    rdfs:comment "Chapter 87 Vehicles other than railway or tramway rolling stock and parts and accessories thereof - GraphNodeID: C355"@en-AU ;
    skos:definition "Chapter 87 Vehicles other than railway or tramway rolling stock and parts and accessories thereof"@en-AU ;
    skos:narrower C2004A04997:317 ;
    skos:prefLabel "Chapter C355"@en-AU ;
    dcat:accessURL "https://www.legislation.gov.au/C2004A04997/2024-07-01/2024-07-01/text/1/epub/OEBPS/document_5/document_5.html#_Toc171753197"^^xsd:anyURI .

C2004A04997:356 a legcons:Item,
        skos:Concept,
        dcat:Resource ;
    rdfs:label "Item I356"@en-AU ;
    rdfs:comment "Notes - GraphNodeID: I356"@en-AU ;
    skos:definition "Notes"@en-AU ;
    skos:narrower C2004A04997:56 ;
    skos:prefLabel "Item I356"@en-AU ;
    dcat:accessURL "https://www.legislation.gov.au/C2004A04997/2024-07-01/2024-07-01/text/1/epub/OEBPS/document_5/document_5.html#_Toc171753198"^^xsd:anyURI .

C2004A04997:357 a legcons:Item,
        skos:Concept,
        dcat:Resource ;
    rdfs:label "Item I357"@en-AU ;
    rdfs:comment "Subheading Note - GraphNodeID: I357"@en-AU ;
    skos:definition "Subheading Note"@en-AU ;
    skos:narrower C2004A04997:56 ;
    skos:prefLabel "Item I357"@en-AU ;
    dcat:accessURL "https://www.legislation.gov.au/C2004A04997/2024-07-01/2024-07-01/text/1/epub/OEBPS/document_5/document_5.html#_Toc171753199"^^xsd:anyURI .

C2004A04997:358 a legcons:Item,
        skos:Concept,
        dcat:Resource ;
    rdfs:label "Item I358"@en-AU ;
    rdfs:comment "Additional Notes - GraphNodeID: I358"@en-AU ;
    skos:definition "Additional Notes"@en-AU ;
    skos:narrower C2004A04997:56 ;
    skos:prefLabel "Item I358"@en-AU ;
    dcat:accessURL "https://www.legislation.gov.au/C2004A04997/2024-07-01/2024-07-01/text/1/epub/OEBPS/document_5/document_5.html#_Toc171753200"^^xsd:anyURI .

C2004A04997:359 a legcons:Chapter,
        skos:Concept,
        dcat:Resource ;
    rdfs:label "Chapter C359"@en-AU ;
    rdfs:comment "Chapter 88 Aircraft spacecraft and parts thereof - GraphNodeID: C359"@en-AU ;
    skos:definition "Chapter 88 Aircraft spacecraft and parts thereof"@en-AU ;
    skos:narrower C2004A04997:317 ;
    skos:prefLabel "Chapter C359"@en-AU ;
    dcat:accessURL "https://www.legislation.gov.au/C2004A04997/2024-07-01/2024-07-01/text/1/epub/OEBPS/document_5/document_5.html#_Toc171753201"^^xsd:anyURI .

C2004A04997:360 a legcons:Item,
        skos:Concept,
        dcat:Resource ;
    rdfs:label "Item I360"@en-AU ;
    rdfs:comment "Note - GraphNodeID: I360"@en-AU ;
    skos:definition "Note"@en-AU ;
    skos:narrower C2004A04997:56 ;
    skos:prefLabel "Item I360"@en-AU ;
    dcat:accessURL "https://www.legislation.gov.au/C2004A04997/2024-07-01/2024-07-01/text/1/epub/OEBPS/document_5/document_5.html#_Toc171753202"^^xsd:anyURI .

C2004A04997:361 a legcons:Item,
        skos:Concept,
        dcat:Resource ;
    rdfs:label "Item I361"@en-AU ;
    rdfs:comment "Subheading Notes - GraphNodeID: I361"@en-AU ;
    skos:definition "Subheading Notes"@en-AU ;
    skos:narrower C2004A04997:56 ;
    skos:prefLabel "Item I361"@en-AU ;
    dcat:accessURL "https://www.legislation.gov.au/C2004A04997/2024-07-01/2024-07-01/text/1/epub/OEBPS/document_5/document_5.html#_Toc171753203"^^xsd:anyURI .

C2004A04997:362 a legcons:Chapter,
        skos:Concept,
        dcat:Resource ;
    rdfs:label "Chapter C362"@en-AU ;
    rdfs:comment "Chapter 89 Ships boats and floating structures - GraphNodeID: C362"@en-AU ;
    skos:definition "Chapter 89 Ships boats and floating structures"@en-AU ;
    skos:narrower C2004A04997:317 ;
    skos:prefLabel "Chapter C362"@en-AU ;
    dcat:accessURL "https://www.legislation.gov.au/C2004A04997/2024-07-01/2024-07-01/text/1/epub/OEBPS/document_5/document_5.html#_Toc171753204"^^xsd:anyURI .

C2004A04997:363 a legcons:Item,
        skos:Concept,
        dcat:Resource ;
    rdfs:label "Item I363"@en-AU ;
    rdfs:comment "Note - GraphNodeID: I363"@en-AU ;
    skos:definition "Note"@en-AU ;
    skos:narrower C2004A04997:56 ;
    skos:prefLabel "Item I363"@en-AU ;
    dcat:accessURL "https://www.legislation.gov.au/C2004A04997/2024-07-01/2024-07-01/text/1/epub/OEBPS/document_5/document_5.html#_Toc171753205"^^xsd:anyURI .

C2004A04997:364 a legcons:Item,
        skos:Concept,
        dcat:Resource ;
    rdfs:label "Item I364"@en-AU ;
    rdfs:comment "Section XVIIIOptical photographic cinematographic measuring checking precision medical or surgical instruments and apparatus clocks and watches musical instruments parts and accessories thereof - GraphNodeID: I364"@en-AU ;
    skos:definition "Section XVIIIOptical photographic cinematographic measuring checking precision medical or surgical instruments and apparatus clocks and watches musical instruments parts and accessories thereof"@en-AU ;
    skos:narrower C2004A04997:56 ;
    skos:prefLabel "Item I364"@en-AU ;
    dcat:accessURL "https://www.legislation.gov.au/C2004A04997/2024-07-01/2024-07-01/text/1/epub/OEBPS/document_5/document_5.html#_Toc171753206"^^xsd:anyURI .

C2004A04997:365 a legcons:Chapter,
        skos:Concept,
        dcat:Resource ;
    rdfs:label "Chapter C365"@en-AU ;
    rdfs:comment "Chapter 90 Optical photographic cinematographic measuring checking precision medical or surgical instruments and apparatus parts and accessories thereof - GraphNodeID: C365"@en-AU ;
    skos:definition "Chapter 90 Optical photographic cinematographic measuring checking precision medical or surgical instruments and apparatus parts and accessories thereof"@en-AU ;
    skos:narrower C2004A04997:317 ;
    skos:prefLabel "Chapter C365"@en-AU ;
    dcat:accessURL "https://www.legislation.gov.au/C2004A04997/2024-07-01/2024-07-01/text/1/epub/OEBPS/document_5/document_5.html#_Toc171753207"^^xsd:anyURI .

C2004A04997:366 a legcons:Item,
        skos:Concept,
        dcat:Resource ;
    rdfs:label "Item I366"@en-AU ;
    rdfs:comment "Notes - GraphNodeID: I366"@en-AU ;
    skos:definition "Notes"@en-AU ;
    skos:narrower C2004A04997:56 ;
    skos:prefLabel "Item I366"@en-AU ;
    dcat:accessURL "https://www.legislation.gov.au/C2004A04997/2024-07-01/2024-07-01/text/1/epub/OEBPS/document_5/document_5.html#_Toc171753208"^^xsd:anyURI .

C2004A04997:367 a legcons:Item,
        skos:Concept,
        dcat:Resource ;
    rdfs:label "Item I367"@en-AU ;
    rdfs:comment "Additional Notes - GraphNodeID: I367"@en-AU ;
    skos:definition "Additional Notes"@en-AU ;
    skos:narrower C2004A04997:56 ;
    skos:prefLabel "Item I367"@en-AU ;
    dcat:accessURL "https://www.legislation.gov.au/C2004A04997/2024-07-01/2024-07-01/text/1/epub/OEBPS/document_5/document_5.html#_Toc171753209"^^xsd:anyURI .

C2004A04997:368 a legcons:Chapter,
        skos:Concept,
        dcat:Resource ;
    rdfs:label "Chapter C368"@en-AU ;
    rdfs:comment "Chapter 91 Clocks and watches and parts thereof - GraphNodeID: C368"@en-AU ;
    skos:definition "Chapter 91 Clocks and watches and parts thereof"@en-AU ;
    skos:narrower C2004A04997:317 ;
    skos:prefLabel "Chapter C368"@en-AU ;
    dcat:accessURL "https://www.legislation.gov.au/C2004A04997/2024-07-01/2024-07-01/text/1/epub/OEBPS/document_5/document_5.html#_Toc171753210"^^xsd:anyURI .

C2004A04997:369 a legcons:Item,
        skos:Concept,
        dcat:Resource ;
    rdfs:label "Item I369"@en-AU ;
    rdfs:comment "Notes - GraphNodeID: I369"@en-AU ;
    skos:definition "Notes"@en-AU ;
    skos:narrower C2004A04997:56 ;
    skos:prefLabel "Item I369"@en-AU ;
    dcat:accessURL "https://www.legislation.gov.au/C2004A04997/2024-07-01/2024-07-01/text/1/epub/OEBPS/document_5/document_5.html#_Toc171753211"^^xsd:anyURI .

C2004A04997:37 a legcons:Item,
        skos:Concept,
        dcat:Resource ;
    rdfs:label "Item I37"@en-AU ;
    rdfs:comment "15  Imposition of duties - GraphNodeID: I37"@en-AU ;
    skos:definition "15  Imposition of duties"@en-AU ;
    skos:narrower C2004A04997:36 ;
    skos:prefLabel "Item I37"@en-AU ;
    dcat:accessURL "https://www.legislation.gov.au/C2004A04997/2024-07-01/2024-07-01/text/1/epub/OEBPS/document_1/document_1.html#_Toc172806537"^^xsd:anyURI .

C2004A04997:370 a legcons:Chapter,
        skos:Concept,
        dcat:Resource ;
    rdfs:label "Chapter C370"@en-AU ;
    rdfs:comment "Chapter 92 Musical instruments parts and accessories of such articles - GraphNodeID: C370"@en-AU ;
    skos:definition "Chapter 92 Musical instruments parts and accessories of such articles"@en-AU ;
    skos:narrower C2004A04997:317 ;
    skos:prefLabel "Chapter C370"@en-AU ;
    dcat:accessURL "https://www.legislation.gov.au/C2004A04997/2024-07-01/2024-07-01/text/1/epub/OEBPS/document_5/document_5.html#_Toc171753212"^^xsd:anyURI .

C2004A04997:371 a legcons:Item,
        skos:Concept,
        dcat:Resource ;
    rdfs:label "Item I371"@en-AU ;
    rdfs:comment "Notes - GraphNodeID: I371"@en-AU ;
    skos:definition "Notes"@en-AU ;
    skos:narrower C2004A04997:56 ;
    skos:prefLabel "Item I371"@en-AU ;
    dcat:accessURL "https://www.legislation.gov.au/C2004A04997/2024-07-01/2024-07-01/text/1/epub/OEBPS/document_5/document_5.html#_Toc171753213"^^xsd:anyURI .

C2004A04997:372 a legcons:Item,
        skos:Concept,
        dcat:Resource ;
    rdfs:label "Item I372"@en-AU ;
    rdfs:comment "Section XIXArms and ammunition parts and accessories thereof - GraphNodeID: I372"@en-AU ;
    skos:definition "Section XIXArms and ammunition parts and accessories thereof"@en-AU ;
    skos:narrower C2004A04997:56 ;
    skos:prefLabel "Item I372"@en-AU ;
    dcat:accessURL "https://www.legislation.gov.au/C2004A04997/2024-07-01/2024-07-01/text/1/epub/OEBPS/document_5/document_5.html#_Toc171753214"^^xsd:anyURI .

C2004A04997:373 a legcons:Chapter,
        skos:Concept,
        dcat:Resource ;
    rdfs:label "Chapter C373"@en-AU ;
    rdfs:comment "Chapter 93 Arms and ammunition parts and accessories thereof - GraphNodeID: C373"@en-AU ;
    skos:definition "Chapter 93 Arms and ammunition parts and accessories thereof"@en-AU ;
    skos:narrower C2004A04997:317 ;
    skos:prefLabel "Chapter C373"@en-AU ;
    dcat:accessURL "https://www.legislation.gov.au/C2004A04997/2024-07-01/2024-07-01/text/1/epub/OEBPS/document_5/document_5.html#_Toc171753215"^^xsd:anyURI .

C2004A04997:374 a legcons:Item,
        skos:Concept,
        dcat:Resource ;
    rdfs:label "Item I374"@en-AU ;
    rdfs:comment "Notes - GraphNodeID: I374"@en-AU ;
    skos:definition "Notes"@en-AU ;
    skos:narrower C2004A04997:56 ;
    skos:prefLabel "Item I374"@en-AU ;
    dcat:accessURL "https://www.legislation.gov.au/C2004A04997/2024-07-01/2024-07-01/text/1/epub/OEBPS/document_5/document_5.html#_Toc171753216"^^xsd:anyURI .

C2004A04997:375 a legcons:Item,
        skos:Concept,
        dcat:Resource ;
    rdfs:label "Item I375"@en-AU ;
    rdfs:comment "Section XXMiscellaneous manufactured articles - GraphNodeID: I375"@en-AU ;
    skos:definition "Section XXMiscellaneous manufactured articles"@en-AU ;
    skos:narrower C2004A04997:56 ;
    skos:prefLabel "Item I375"@en-AU ;
    dcat:accessURL "https://www.legislation.gov.au/C2004A04997/2024-07-01/2024-07-01/text/1/epub/OEBPS/document_5/document_5.html#_Toc171753217"^^xsd:anyURI .

C2004A04997:376 a legcons:Chapter,
        skos:Concept,
        dcat:Resource ;
    rdfs:label "Chapter C376"@en-AU ;
    rdfs:comment "Chapter 94 Furniture bedding mattresses mattress supports cushions and similar stuffed furnishings luminaires and lighting fittings not elsewhere specified or included illuminated signs illuminated name plates and the like prefabricated buildings - GraphNodeID: C376"@en-AU ;
    skos:definition "Chapter 94 Furniture bedding mattresses mattress supports cushions and similar stuffed furnishings luminaires and lighting fittings not elsewhere specified or included illuminated signs illuminated name plates and the like prefabricated buildings"@en-AU ;
    skos:narrower C2004A04997:317 ;
    skos:prefLabel "Chapter C376"@en-AU ;
    dcat:accessURL "https://www.legislation.gov.au/C2004A04997/2024-07-01/2024-07-01/text/1/epub/OEBPS/document_5/document_5.html#_Toc171753218"^^xsd:anyURI .

C2004A04997:377 a legcons:Item,
        skos:Concept,
        dcat:Resource ;
    rdfs:label "Item I377"@en-AU ;
    rdfs:comment "Notes - GraphNodeID: I377"@en-AU ;
    skos:definition "Notes"@en-AU ;
    skos:narrower C2004A04997:56 ;
    skos:prefLabel "Item I377"@en-AU ;
    dcat:accessURL "https://www.legislation.gov.au/C2004A04997/2024-07-01/2024-07-01/text/1/epub/OEBPS/document_5/document_5.html#_Toc171753219"^^xsd:anyURI .

C2004A04997:378 a legcons:Item,
        skos:Concept,
        dcat:Resource ;
    rdfs:label "Item I378"@en-AU ;
    rdfs:comment "Additional Note - GraphNodeID: I378"@en-AU ;
    skos:definition "Additional Note"@en-AU ;
    skos:narrower C2004A04997:56 ;
    skos:prefLabel "Item I378"@en-AU ;
    dcat:accessURL "https://www.legislation.gov.au/C2004A04997/2024-07-01/2024-07-01/text/1/epub/OEBPS/document_5/document_5.html#_Toc171753220"^^xsd:anyURI .

C2004A04997:379 a legcons:Chapter,
        skos:Concept,
        dcat:Resource ;
    rdfs:label "Chapter C379"@en-AU ;
    rdfs:comment "Chapter 95 Toys games and sports requisites parts and accessories thereof - GraphNodeID: C379"@en-AU ;
    skos:definition "Chapter 95 Toys games and sports requisites parts and accessories thereof"@en-AU ;
    skos:narrower C2004A04997:317 ;
    skos:prefLabel "Chapter C379"@en-AU ;
    dcat:accessURL "https://www.legislation.gov.au/C2004A04997/2024-07-01/2024-07-01/text/1/epub/OEBPS/document_5/document_5.html#_Toc171753221"^^xsd:anyURI .

C2004A04997:38 a legcons:Item,
        skos:Concept,
        dcat:Resource ;
    rdfs:label "Item I38"@en-AU ;
    rdfs:comment "16  Calculation of duty - GraphNodeID: I38"@en-AU ;
    skos:definition "16  Calculation of duty"@en-AU ;
    skos:narrower C2004A04997:36 ;
    skos:prefLabel "Item I38"@en-AU ;
    dcat:accessURL "https://www.legislation.gov.au/C2004A04997/2024-07-01/2024-07-01/text/1/epub/OEBPS/document_1/document_1.html#_Toc172806538"^^xsd:anyURI .

C2004A04997:380 a legcons:Item,
        skos:Concept,
        dcat:Resource ;
    rdfs:label "Item I380"@en-AU ;
    rdfs:comment "Notes - GraphNodeID: I380"@en-AU ;
    skos:definition "Notes"@en-AU ;
    skos:narrower C2004A04997:56 ;
    skos:prefLabel "Item I380"@en-AU ;
    dcat:accessURL "https://www.legislation.gov.au/C2004A04997/2024-07-01/2024-07-01/text/1/epub/OEBPS/document_5/document_5.html#_Toc171753222"^^xsd:anyURI .

C2004A04997:381 a legcons:Item,
        skos:Concept,
        dcat:Resource ;
    rdfs:label "Item I381"@en-AU ;
    rdfs:comment "Subheading Note - GraphNodeID: I381"@en-AU ;
    skos:definition "Subheading Note"@en-AU ;
    skos:narrower C2004A04997:56 ;
    skos:prefLabel "Item I381"@en-AU ;
    dcat:accessURL "https://www.legislation.gov.au/C2004A04997/2024-07-01/2024-07-01/text/1/epub/OEBPS/document_5/document_5.html#_Toc171753223"^^xsd:anyURI .

C2004A04997:382 a legcons:Chapter,
        skos:Concept,
        dcat:Resource ;
    rdfs:label "Chapter C382"@en-AU ;
    rdfs:comment "Chapter 96 Miscellaneous manufactured articles - GraphNodeID: C382"@en-AU ;
    skos:definition "Chapter 96 Miscellaneous manufactured articles"@en-AU ;
    skos:narrower C2004A04997:317 ;
    skos:prefLabel "Chapter C382"@en-AU ;
    dcat:accessURL "https://www.legislation.gov.au/C2004A04997/2024-07-01/2024-07-01/text/1/epub/OEBPS/document_5/document_5.html#_Toc171753224"^^xsd:anyURI .

C2004A04997:383 a legcons:Item,
        skos:Concept,
        dcat:Resource ;
    rdfs:label "Item I383"@en-AU ;
    rdfs:comment "Notes - GraphNodeID: I383"@en-AU ;
    skos:definition "Notes"@en-AU ;
    skos:narrower C2004A04997:56 ;
    skos:prefLabel "Item I383"@en-AU ;
    dcat:accessURL "https://www.legislation.gov.au/C2004A04997/2024-07-01/2024-07-01/text/1/epub/OEBPS/document_5/document_5.html#_Toc171753225"^^xsd:anyURI .

C2004A04997:384 a legcons:Item,
        skos:Concept,
        dcat:Resource ;
    rdfs:label "Item I384"@en-AU ;
    rdfs:comment "Section XXIWorks of art collectors pieces and antiques - GraphNodeID: I384"@en-AU ;
    skos:definition "Section XXIWorks of art collectors pieces and antiques"@en-AU ;
    skos:narrower C2004A04997:56 ;
    skos:prefLabel "Item I384"@en-AU ;
    dcat:accessURL "https://www.legislation.gov.au/C2004A04997/2024-07-01/2024-07-01/text/1/epub/OEBPS/document_5/document_5.html#_Toc171753226"^^xsd:anyURI .

C2004A04997:386 a legcons:Item,
        skos:Concept,
        dcat:Resource ;
    rdfs:label "Item I386"@en-AU ;
    rdfs:comment "Notes - GraphNodeID: I386"@en-AU ;
    skos:definition "Notes"@en-AU ;
    skos:narrower C2004A04997:56 ;
    skos:prefLabel "Item I386"@en-AU ;
    dcat:accessURL "https://www.legislation.gov.au/C2004A04997/2024-07-01/2024-07-01/text/1/epub/OEBPS/document_5/document_5.html#_Toc171753228"^^xsd:anyURI .

C2004A04997:387 a legcons:Item,
        skos:Concept,
        dcat:Resource ;
    rdfs:label "Item I387"@en-AU ;
    rdfs:comment "Additional Notes - GraphNodeID: I387"@en-AU ;
    skos:definition "Additional Notes"@en-AU ;
    skos:narrower C2004A04997:56 ;
    skos:prefLabel "Item I387"@en-AU ;
    dcat:accessURL "https://www.legislation.gov.au/C2004A04997/2024-07-01/2024-07-01/text/1/epub/OEBPS/document_5/document_5.html#_Toc171753229"^^xsd:anyURI .

C2004A04997:389 a legcons:Item,
        skos:Concept,
        dcat:Resource ;
    rdfs:label "Item I389"@en-AU ;
    rdfs:comment "Schedule 4 Concessional rates of duty - GraphNodeID: I389"@en-AU ;
    skos:definition "Schedule 4 Concessional rates of duty"@en-AU ;
    skos:narrower C2004A04997:56 ;
    skos:prefLabel "Item I389"@en-AU ;
    dcat:accessURL "https://www.legislation.gov.au/C2004A04997/2024-07-01/2024-07-01/text/1/epub/OEBPS/document_6/document_6.html#_Toc171754999"^^xsd:anyURI .

C2004A04997:39 a legcons:Item,
        skos:Concept,
        dcat:Resource ;
    rdfs:label "Item I39"@en-AU ;
    rdfs:comment "16 A  Suspension of preferential tariff for UK originating goodssafeguard goods - GraphNodeID: I39"@en-AU ;
    skos:definition "16 A  Suspension of preferential tariff for UK originating goodssafeguard goods"@en-AU ;
    skos:narrower C2004A04997:36 ;
    skos:prefLabel "Item I39"@en-AU ;
    dcat:accessURL "https://www.legislation.gov.au/C2004A04997/2024-07-01/2024-07-01/text/1/epub/OEBPS/document_1/document_1.html#_Toc172806539"^^xsd:anyURI .

C2004A04997:390 a legcons:Item,
        skos:Concept,
        dcat:Resource ;
    rdfs:label "Item I390"@en-AU ;
    rdfs:comment "Schedule 4 ASingaporean originating goods - GraphNodeID: I390"@en-AU ;
    skos:definition "Schedule 4 ASingaporean originating goods"@en-AU ;
    skos:narrower C2004A04997:56 ;
    skos:prefLabel "Item I390"@en-AU ;
    dcat:accessURL "https://www.legislation.gov.au/C2004A04997/2024-07-01/2024-07-01/text/1/epub/OEBPS/document_6/document_6.html#_Toc171755000"^^xsd:anyURI .

C2004A04997:391 a legcons:Item,
        skos:Concept,
        dcat:Resource ;
    rdfs:label "Item I391"@en-AU ;
    rdfs:comment "Schedule 5 US originating goods - GraphNodeID: I391"@en-AU ;
    skos:definition "Schedule 5 US originating goods"@en-AU ;
    skos:narrower C2004A04997:56 ;
    skos:prefLabel "Item I391"@en-AU ;
    dcat:accessURL "https://www.legislation.gov.au/C2004A04997/2024-07-01/2024-07-01/text/1/epub/OEBPS/document_6/document_6.html#_Toc171755001"^^xsd:anyURI .

C2004A04997:392 a legcons:Item,
        skos:Concept,
        dcat:Resource ;
    rdfs:label "Item I392"@en-AU ;
    rdfs:comment "Schedule 6 Thai originating goods - GraphNodeID: I392"@en-AU ;
    skos:definition "Schedule 6 Thai originating goods"@en-AU ;
    skos:narrower C2004A04997:56 ;
    skos:prefLabel "Item I392"@en-AU ;
    dcat:accessURL "https://www.legislation.gov.au/C2004A04997/2024-07-01/2024-07-01/text/1/epub/OEBPS/document_6/document_6.html#_Toc171755002"^^xsd:anyURI .

C2004A04997:393 a legcons:Item,
        skos:Concept,
        dcat:Resource ;
    rdfs:label "Item I393"@en-AU ;
    rdfs:comment "Schedule 6 APeruvian originating goods - GraphNodeID: I393"@en-AU ;
    skos:definition "Schedule 6 APeruvian originating goods"@en-AU ;
    skos:narrower C2004A04997:56 ;
    skos:prefLabel "Item I393"@en-AU ;
    dcat:accessURL "https://www.legislation.gov.au/C2004A04997/2024-07-01/2024-07-01/text/1/epub/OEBPS/document_6/document_6.html#_Toc171755003"^^xsd:anyURI .

C2004A04997:394 a legcons:Item,
        skos:Concept,
        dcat:Resource ;
    rdfs:label "Item I394"@en-AU ;
    rdfs:comment "Schedule 7 Chilean originating goods - GraphNodeID: I394"@en-AU ;
    skos:definition "Schedule 7 Chilean originating goods"@en-AU ;
    skos:narrower C2004A04997:56 ;
    skos:prefLabel "Item I394"@en-AU ;
    dcat:accessURL "https://www.legislation.gov.au/C2004A04997/2024-07-01/2024-07-01/text/1/epub/OEBPS/document_6/document_6.html#_Toc171755004"^^xsd:anyURI .

C2004A04997:395 a legcons:Item,
        skos:Concept,
        dcat:Resource ;
    rdfs:label "Item I395"@en-AU ;
    rdfs:comment "Schedule 8 ASEAN Australia New Zealand AANZ originating goods - GraphNodeID: I395"@en-AU ;
    skos:definition "Schedule 8 ASEAN Australia New Zealand AANZ originating goods"@en-AU ;
    skos:narrower C2004A04997:56 ;
    skos:prefLabel "Item I395"@en-AU ;
    dcat:accessURL "https://www.legislation.gov.au/C2004A04997/2024-07-01/2024-07-01/text/1/epub/OEBPS/document_6/document_6.html#_Toc171755005"^^xsd:anyURI .

C2004A04997:396 a legcons:Item,
        skos:Concept,
        dcat:Resource ;
    rdfs:label "Item I396"@en-AU ;
    rdfs:comment "Schedule 8 APacific Islands originating goods - GraphNodeID: I396"@en-AU ;
    skos:definition "Schedule 8 APacific Islands originating goods"@en-AU ;
    skos:narrower C2004A04997:56 ;
    skos:prefLabel "Item I396"@en-AU ;
    dcat:accessURL "https://www.legislation.gov.au/C2004A04997/2024-07-01/2024-07-01/text/1/epub/OEBPS/document_6/document_6.html#_Toc171755006"^^xsd:anyURI .

C2004A04997:397 a legcons:Item,
        skos:Concept,
        dcat:Resource ;
    rdfs:label "Item I397"@en-AU ;
    rdfs:comment "Schedule 8 BTrans Pacific Partnership originating goods - GraphNodeID: I397"@en-AU ;
    skos:definition "Schedule 8 BTrans Pacific Partnership originating goods"@en-AU ;
    skos:narrower C2004A04997:56 ;
    skos:prefLabel "Item I397"@en-AU ;
    dcat:accessURL "https://www.legislation.gov.au/C2004A04997/2024-07-01/2024-07-01/text/1/epub/OEBPS/document_6/document_6.html#_Toc171755007"^^xsd:anyURI .

C2004A04997:398 a legcons:Item,
        skos:Concept,
        dcat:Resource ;
    rdfs:label "Item I398"@en-AU ;
    rdfs:comment "Schedule 9 Malaysian originating goods - GraphNodeID: I398"@en-AU ;
    skos:definition "Schedule 9 Malaysian originating goods"@en-AU ;
    skos:narrower C2004A04997:56 ;
    skos:prefLabel "Item I398"@en-AU ;
    dcat:accessURL "https://www.legislation.gov.au/C2004A04997/2024-07-01/2024-07-01/text/1/epub/OEBPS/document_6/document_6.html#_Toc171755008"^^xsd:anyURI .

C2004A04997:399 a legcons:Item,
        skos:Concept,
        dcat:Resource ;
    rdfs:label "Item I399"@en-AU ;
    rdfs:comment "Schedule 9 AIndonesian originating goods - GraphNodeID: I399"@en-AU ;
    skos:definition "Schedule 9 AIndonesian originating goods"@en-AU ;
    skos:narrower C2004A04997:56 ;
    skos:prefLabel "Item I399"@en-AU ;
    dcat:accessURL "https://www.legislation.gov.au/C2004A04997/2024-07-01/2024-07-01/text/1/epub/OEBPS/document_6/document_6.html#_Toc171755009"^^xsd:anyURI .

C2004A04997:4 a legcons:Item,
        skos:Concept,
        dcat:Resource ;
    rdfs:label "Item I4"@en-AU ;
    rdfs:comment "2  Commencement - GraphNodeID: I4"@en-AU ;
    skos:definition "2  Commencement"@en-AU ;
    skos:narrower C2004A04997:2 ;
    skos:prefLabel "Item I4"@en-AU ;
    dcat:accessURL "https://www.legislation.gov.au/C2004A04997/2024-07-01/2024-07-01/text/1/epub/OEBPS/document_1/document_1.html#_Toc172806504"^^xsd:anyURI .

C2004A04997:40 a legcons:Item,
        skos:Concept,
        dcat:Resource ;
    rdfs:label "Item I40"@en-AU ;
    rdfs:comment "17  Rates for goods with constituents etc - GraphNodeID: I40"@en-AU ;
    skos:definition "17  Rates for goods with constituents etc"@en-AU ;
    skos:narrower C2004A04997:36 ;
    skos:prefLabel "Item I40"@en-AU ;
    dcat:accessURL "https://www.legislation.gov.au/C2004A04997/2024-07-01/2024-07-01/text/1/epub/OEBPS/document_1/document_1.html#_Toc172806540"^^xsd:anyURI .

C2004A04997:400 a legcons:Item,
        skos:Concept,
        dcat:Resource ;
    rdfs:label "Item I400"@en-AU ;
    rdfs:comment "Schedule 10 Korean originating goods - GraphNodeID: I400"@en-AU ;
    skos:definition "Schedule 10 Korean originating goods"@en-AU ;
    skos:narrower C2004A04997:56 ;
    skos:prefLabel "Item I400"@en-AU ;
    dcat:accessURL "https://www.legislation.gov.au/C2004A04997/2024-07-01/2024-07-01/text/1/epub/OEBPS/document_6/document_6.html#_Toc171755010"^^xsd:anyURI .

C2004A04997:401 a legcons:Item,
        skos:Concept,
        dcat:Resource ;
    rdfs:label "Item I401"@en-AU ;
    rdfs:comment "Schedule 10 AIndian originating goods - GraphNodeID: I401"@en-AU ;
    skos:definition "Schedule 10 AIndian originating goods"@en-AU ;
    skos:narrower C2004A04997:56 ;
    skos:prefLabel "Item I401"@en-AU ;
    dcat:accessURL "https://www.legislation.gov.au/C2004A04997/2024-07-01/2024-07-01/text/1/epub/OEBPS/document_6/document_6.html#_Toc171755011"^^xsd:anyURI .

C2004A04997:402 a legcons:Item,
        skos:Concept,
        dcat:Resource ;
    rdfs:label "Item I402"@en-AU ;
    rdfs:comment "Schedule 11 Japanese originating goods - GraphNodeID: I402"@en-AU ;
    skos:definition "Schedule 11 Japanese originating goods"@en-AU ;
    skos:narrower C2004A04997:56 ;
    skos:prefLabel "Item I402"@en-AU ;
    dcat:accessURL "https://www.legislation.gov.au/C2004A04997/2024-07-01/2024-07-01/text/1/epub/OEBPS/document_6/document_6.html#_Toc171755012"^^xsd:anyURI .

C2004A04997:403 a legcons:Item,
        skos:Concept,
        dcat:Resource ;
    rdfs:label "Item I403"@en-AU ;
    rdfs:comment "Schedule 12 Chinese originating goods - GraphNodeID: I403"@en-AU ;
    skos:definition "Schedule 12 Chinese originating goods"@en-AU ;
    skos:narrower C2004A04997:56 ;
    skos:prefLabel "Item I403"@en-AU ;
    dcat:accessURL "https://www.legislation.gov.au/C2004A04997/2024-07-01/2024-07-01/text/1/epub/OEBPS/document_6/document_6.html#_Toc171755013"^^xsd:anyURI .

C2004A04997:404 a legcons:Item,
        skos:Concept,
        dcat:Resource ;
    rdfs:label "Item I404"@en-AU ;
    rdfs:comment "Schedule 13 Hong Kong originating goods - GraphNodeID: I404"@en-AU ;
    skos:definition "Schedule 13 Hong Kong originating goods"@en-AU ;
    skos:narrower C2004A04997:56 ;
    skos:prefLabel "Item I404"@en-AU ;
    dcat:accessURL "https://www.legislation.gov.au/C2004A04997/2024-07-01/2024-07-01/text/1/epub/OEBPS/document_6/document_6.html#_Toc171755014"^^xsd:anyURI .

C2004A04997:405 a legcons:Item,
        skos:Concept,
        dcat:Resource ;
    rdfs:label "Item I405"@en-AU ;
    rdfs:comment "Schedule 14 Regional Comprehensive Economic Partnership RCEP originating goods - GraphNodeID: I405"@en-AU ;
    skos:definition "Schedule 14 Regional Comprehensive Economic Partnership RCEP originating goods"@en-AU ;
    skos:narrower C2004A04997:56 ;
    skos:prefLabel "Item I405"@en-AU ;
    dcat:accessURL "https://www.legislation.gov.au/C2004A04997/2024-07-01/2024-07-01/text/1/epub/OEBPS/document_6/document_6.html#_Toc171755015"^^xsd:anyURI .

C2004A04997:406 a legcons:Item,
        skos:Concept,
        dcat:Resource ;
    rdfs:label "Item I406"@en-AU ;
    rdfs:comment "Schedule 15 UK originating goods - GraphNodeID: I406"@en-AU ;
    skos:definition "Schedule 15 UK originating goods"@en-AU ;
    skos:narrower C2004A04997:56 ;
    skos:prefLabel "Item I406"@en-AU ;
    dcat:accessURL "https://www.legislation.gov.au/C2004A04997/2024-07-01/2024-07-01/text/1/epub/OEBPS/document_6/document_6.html#_Toc171755016"^^xsd:anyURI .

C2004A04997:409 a legcons:Item,
        skos:Concept,
        dcat:Resource ;
    rdfs:label "Item I409"@en-AU ;
    rdfs:comment "Endnote 1 About the endnotes - GraphNodeID: I409"@en-AU ;
    skos:definition "Endnote 1 About the endnotes"@en-AU ;
    skos:narrower C2004A04997:408 ;
    skos:prefLabel "Item I409"@en-AU ;
    dcat:accessURL "https://www.legislation.gov.au/C2004A04997/2024-07-01/2024-07-01/text/1/epub/OEBPS/document_7/document_7.html#_Toc171755739"^^xsd:anyURI .

C2004A04997:41 a legcons:Item,
        skos:Concept,
        dcat:Resource ;
    rdfs:label "Item I41"@en-AU ;
    rdfs:comment "18  Calculation of concessional duty - GraphNodeID: I41"@en-AU ;
    skos:definition "18  Calculation of concessional duty"@en-AU ;
    skos:narrower C2004A04997:36 ;
    skos:prefLabel "Item I41"@en-AU ;
    dcat:accessURL "https://www.legislation.gov.au/C2004A04997/2024-07-01/2024-07-01/text/1/epub/OEBPS/document_1/document_1.html#_Toc172806541"^^xsd:anyURI .

C2004A04997:410 a legcons:Item,
        skos:Concept,
        dcat:Resource ;
    rdfs:label "Item I410"@en-AU ;
    rdfs:comment "Endnote 2 Abbreviation key - GraphNodeID: I410"@en-AU ;
    skos:definition "Endnote 2 Abbreviation key"@en-AU ;
    skos:narrower C2004A04997:408 ;
    skos:prefLabel "Item I410"@en-AU ;
    dcat:accessURL "https://www.legislation.gov.au/C2004A04997/2024-07-01/2024-07-01/text/1/epub/OEBPS/document_7/document_7.html#_Toc171755740"^^xsd:anyURI .

C2004A04997:411 a legcons:Item,
        skos:Concept,
        dcat:Resource ;
    rdfs:label "Item I411"@en-AU ;
    rdfs:comment "Endnote 3 Legislation history - GraphNodeID: I411"@en-AU ;
    skos:definition "Endnote 3 Legislation history"@en-AU ;
    skos:narrower C2004A04997:408 ;
    skos:prefLabel "Item I411"@en-AU ;
    dcat:accessURL "https://www.legislation.gov.au/C2004A04997/2024-07-01/2024-07-01/text/1/epub/OEBPS/document_7/document_7.html#_Toc171755741"^^xsd:anyURI .

C2004A04997:412 a legcons:Item,
        skos:Concept,
        dcat:Resource ;
    rdfs:label "Item I412"@en-AU ;
    rdfs:comment "Endnote 4 Amendment history - GraphNodeID: I412"@en-AU ;
    skos:definition "Endnote 4 Amendment history"@en-AU ;
    skos:narrower C2004A04997:408 ;
    skos:prefLabel "Item I412"@en-AU ;
    dcat:accessURL "https://www.legislation.gov.au/C2004A04997/2024-07-01/2024-07-01/text/1/epub/OEBPS/document_7/document_7.html#_Toc171755742"^^xsd:anyURI .

C2004A04997:42 a legcons:Item,
        skos:Concept,
        dcat:Resource ;
    rdfs:label "Item I42"@en-AU ;
    rdfs:comment "18 A  Temporary increase in duties for goods from Russia or Belarus - GraphNodeID: I42"@en-AU ;
    skos:definition "18 A  Temporary increase in duties for goods from Russia or Belarus"@en-AU ;
    skos:narrower C2004A04997:36 ;
    skos:prefLabel "Item I42"@en-AU ;
    dcat:accessURL "https://www.legislation.gov.au/C2004A04997/2024-07-01/2024-07-01/text/1/epub/OEBPS/document_1/document_1.html#_Toc172806542"^^xsd:anyURI .

C2004A04997:43 a legcons:Item,
        skos:Concept,
        dcat:Resource ;
    rdfs:label "Item I43"@en-AU ;
    rdfs:comment "18 B  Temporary decrease in duties for goods from Ukraine - GraphNodeID: I43"@en-AU ;
    skos:definition "18 B  Temporary decrease in duties for goods from Ukraine"@en-AU ;
    skos:narrower C2004A04997:36 ;
    skos:prefLabel "Item I43"@en-AU ;
    dcat:accessURL "https://www.legislation.gov.au/C2004A04997/2024-07-01/2024-07-01/text/1/epub/OEBPS/document_1/document_1.html#_Toc172806543"^^xsd:anyURI .

C2004A04997:44 a legcons:Item,
        skos:Concept,
        dcat:Resource ;
    rdfs:label "Item I44"@en-AU ;
    rdfs:comment "19  Indexation of CPI indexed rates - GraphNodeID: I44"@en-AU ;
    skos:definition "19  Indexation of CPI indexed rates"@en-AU ;
    skos:narrower C2004A04997:36 ;
    skos:prefLabel "Item I44"@en-AU ;
    dcat:accessURL "https://www.legislation.gov.au/C2004A04997/2024-07-01/2024-07-01/text/1/epub/OEBPS/document_1/document_1.html#_Toc172806544"^^xsd:anyURI .

C2004A04997:45 a legcons:Item,
        skos:Concept,
        dcat:Resource ;
    rdfs:label "Item I45"@en-AU ;
    rdfs:comment "19 AAA  Rounding of fuel duty rates - GraphNodeID: I45"@en-AU ;
    skos:definition "19 AAA  Rounding of fuel duty rates"@en-AU ;
    skos:narrower C2004A04997:36 ;
    skos:prefLabel "Item I45"@en-AU ;
    dcat:accessURL "https://www.legislation.gov.au/C2004A04997/2024-07-01/2024-07-01/text/1/epub/OEBPS/document_1/document_1.html#_Toc172806545"^^xsd:anyURI .

C2004A04997:46 a legcons:Item,
        skos:Concept,
        dcat:Resource ;
    rdfs:label "Item I46"@en-AU ;
    rdfs:comment "19 AAB  Change in fuel duty rates - GraphNodeID: I46"@en-AU ;
    skos:definition "19 AAB  Change in fuel duty rates"@en-AU ;
    skos:narrower C2004A04997:36 ;
    skos:prefLabel "Item I46"@en-AU ;
    dcat:accessURL "https://www.legislation.gov.au/C2004A04997/2024-07-01/2024-07-01/text/1/epub/OEBPS/document_1/document_1.html#_Toc172806546"^^xsd:anyURI .

C2004A04997:47 a legcons:Item,
        skos:Concept,
        dcat:Resource ;
    rdfs:label "Item I47"@en-AU ;
    rdfs:comment "19 AABA  Temporary reduction in indexed fuel duty rates - GraphNodeID: I47"@en-AU ;
    skos:definition "19 AABA  Temporary reduction in indexed fuel duty rates"@en-AU ;
    skos:narrower C2004A04997:36 ;
    skos:prefLabel "Item I47"@en-AU ;
    dcat:accessURL "https://www.legislation.gov.au/C2004A04997/2024-07-01/2024-07-01/text/1/epub/OEBPS/document_1/document_1.html#_Toc172806547"^^xsd:anyURI .

C2004A04997:48 a legcons:Item,
        skos:Concept,
        dcat:Resource ;
    rdfs:label "Item I48"@en-AU ;
    rdfs:comment "19 AABB  Temporary reduction in other duty rates - GraphNodeID: I48"@en-AU ;
    skos:definition "19 AABB  Temporary reduction in other duty rates"@en-AU ;
    skos:narrower C2004A04997:36 ;
    skos:prefLabel "Item I48"@en-AU ;
    dcat:accessURL "https://www.legislation.gov.au/C2004A04997/2024-07-01/2024-07-01/text/1/epub/OEBPS/document_1/document_1.html#_Toc172806548"^^xsd:anyURI .

C2004A04997:49 a legcons:Item,
        skos:Concept,
        dcat:Resource ;
    rdfs:label "Item I49"@en-AU ;
    rdfs:comment "19 AAC  Fuel duty rates - GraphNodeID: I49"@en-AU ;
    skos:definition "19 AAC  Fuel duty rates"@en-AU ;
    skos:narrower C2004A04997:36 ;
    skos:prefLabel "Item I49"@en-AU ;
    dcat:accessURL "https://www.legislation.gov.au/C2004A04997/2024-07-01/2024-07-01/text/1/epub/OEBPS/document_1/document_1.html#_Toc172806549"^^xsd:anyURI .

C2004A04997:5 a legcons:Item,
        skos:Concept,
        dcat:Resource ;
    rdfs:label "Item I5"@en-AU ;
    rdfs:comment "3  Definitions - GraphNodeID: I5"@en-AU ;
    skos:definition "3  Definitions"@en-AU ;
    skos:narrower C2004A04997:2 ;
    skos:prefLabel "Item I5"@en-AU ;
    dcat:accessURL "https://www.legislation.gov.au/C2004A04997/2024-07-01/2024-07-01/text/1/epub/OEBPS/document_1/document_1.html#_Toc172806505"^^xsd:anyURI .

C2004A04997:50 a legcons:Item,
        skos:Concept,
        dcat:Resource ;
    rdfs:label "Item I50"@en-AU ;
    rdfs:comment "19 AA  Alcohol duty rates - GraphNodeID: I50"@en-AU ;
    skos:definition "19 AA  Alcohol duty rates"@en-AU ;
    skos:narrower C2004A04997:36 ;
    skos:prefLabel "Item I50"@en-AU ;
    dcat:accessURL "https://www.legislation.gov.au/C2004A04997/2024-07-01/2024-07-01/text/1/epub/OEBPS/document_1/document_1.html#_Toc172806550"^^xsd:anyURI .

C2004A04997:51 a legcons:Item,
        skos:Concept,
        dcat:Resource ;
    rdfs:label "Item I51"@en-AU ;
    rdfs:comment "19 AB  Indexation of tobacco duty rates - GraphNodeID: I51"@en-AU ;
    skos:definition "19 AB  Indexation of tobacco duty rates"@en-AU ;
    skos:narrower C2004A04997:36 ;
    skos:prefLabel "Item I51"@en-AU ;
    dcat:accessURL "https://www.legislation.gov.au/C2004A04997/2024-07-01/2024-07-01/text/1/epub/OEBPS/document_1/document_1.html#_Toc172806551"^^xsd:anyURI .

C2004A04997:52 a legcons:Item,
        skos:Concept,
        dcat:Resource ;
    rdfs:label "Item I52"@en-AU ;
    rdfs:comment "19 AC  List of tobacco duty rates to be indexed under section 19 AB - GraphNodeID: I52"@en-AU ;
    skos:definition "19 AC  List of tobacco duty rates to be indexed under section 19 AB"@en-AU ;
    skos:narrower C2004A04997:36 ;
    skos:prefLabel "Item I52"@en-AU ;
    dcat:accessURL "https://www.legislation.gov.au/C2004A04997/2024-07-01/2024-07-01/text/1/epub/OEBPS/document_1/document_1.html#_Toc172806552"^^xsd:anyURI .

C2004A04997:53 a legcons:Item,
        skos:Concept,
        dcat:Resource ;
    rdfs:label "Item I53"@en-AU ;
    rdfs:comment "19 ACA  Other tobacco duty rates - GraphNodeID: I53"@en-AU ;
    skos:definition "19 ACA  Other tobacco duty rates"@en-AU ;
    skos:narrower C2004A04997:36 ;
    skos:prefLabel "Item I53"@en-AU ;
    dcat:accessURL "https://www.legislation.gov.au/C2004A04997/2024-07-01/2024-07-01/text/1/epub/OEBPS/document_1/document_1.html#_Toc172806553"^^xsd:anyURI .

C2004A04997:54 a legcons:Item,
        skos:Concept,
        dcat:Resource ;
    rdfs:label "Item I54"@en-AU ;
    rdfs:comment "19 AD  Change in duty rate of certain liquefied petroleum gases liquefied natural gases and compressed natural gases - GraphNodeID: I54"@en-AU ;
    skos:definition "19 AD  Change in duty rate of certain liquefied petroleum gases liquefied natural gases and compressed natural gases"@en-AU ;
    skos:narrower C2004A04997:36 ;
    skos:prefLabel "Item I54"@en-AU ;
    dcat:accessURL "https://www.legislation.gov.au/C2004A04997/2024-07-01/2024-07-01/text/1/epub/OEBPS/document_1/document_1.html#_Toc172806554"^^xsd:anyURI .

C2004A04997:55 a legcons:Item,
        skos:Concept,
        dcat:Resource ;
    rdfs:label "Item I55"@en-AU ;
    rdfs:comment "20  Duty where goods consist of certain containers and certain contents - GraphNodeID: I55"@en-AU ;
    skos:definition "20  Duty where goods consist of certain containers and certain contents"@en-AU ;
    skos:narrower C2004A04997:36 ;
    skos:prefLabel "Item I55"@en-AU ;
    dcat:accessURL "https://www.legislation.gov.au/C2004A04997/2024-07-01/2024-07-01/text/1/epub/OEBPS/document_1/document_1.html#_Toc172806555"^^xsd:anyURI .

C2004A04997:57 a legcons:Item,
        skos:Concept,
        dcat:Resource ;
    rdfs:label "Item I57"@en-AU ;
    rdfs:comment "20 A  Regulations - GraphNodeID: I57"@en-AU ;
    skos:definition "20 A  Regulations"@en-AU ;
    skos:narrower C2004A04997:56 ;
    skos:prefLabel "Item I57"@en-AU ;
    dcat:accessURL "https://www.legislation.gov.au/C2004A04997/2024-07-01/2024-07-01/text/1/epub/OEBPS/document_1/document_1.html#_Toc172806557"^^xsd:anyURI .

C2004A04997:58 a legcons:Item,
        skos:Concept,
        dcat:Resource ;
    rdfs:label "Item I58"@en-AU ;
    rdfs:comment "21  Repeal of the Customs Tariff Act 1987 etc - GraphNodeID: I58"@en-AU ;
    skos:definition "21  Repeal of the Customs Tariff Act 1987 etc"@en-AU ;
    skos:narrower C2004A04997:56 ;
    skos:prefLabel "Item I58"@en-AU ;
    dcat:accessURL "https://www.legislation.gov.au/C2004A04997/2024-07-01/2024-07-01/text/1/epub/OEBPS/document_1/document_1.html#_Toc172806558"^^xsd:anyURI .

C2004A04997:59 a legcons:Item,
        skos:Concept,
        dcat:Resource ;
    rdfs:label "Item I59"@en-AU ;
    rdfs:comment "22  Transitional - GraphNodeID: I59"@en-AU ;
    skos:definition "22  Transitional"@en-AU ;
    skos:narrower C2004A04997:56 ;
    skos:prefLabel "Item I59"@en-AU ;
    dcat:accessURL "https://www.legislation.gov.au/C2004A04997/2024-07-01/2024-07-01/text/1/epub/OEBPS/document_1/document_1.html#_Toc172806559"^^xsd:anyURI .

C2004A04997:6 a legcons:Item,
        skos:Concept,
        dcat:Resource ;
    rdfs:label "Item I6"@en-AU ;
    rdfs:comment "3 A  Act does not extend to Norfolk Island - GraphNodeID: I6"@en-AU ;
    skos:definition "3 A  Act does not extend to Norfolk Island"@en-AU ;
    skos:narrower C2004A04997:2 ;
    skos:prefLabel "Item I6"@en-AU ;
    dcat:accessURL "https://www.legislation.gov.au/C2004A04997/2024-07-01/2024-07-01/text/1/epub/OEBPS/document_1/document_1.html#_Toc172806506"^^xsd:anyURI .

C2004A04997:60 a legcons:Item,
        skos:Concept,
        dcat:Resource ;
    rdfs:label "Item I60"@en-AU ;
    rdfs:comment "Schedule 2 General rules for the interpretation of Schedule 3 - GraphNodeID: I60"@en-AU ;
    skos:definition "Schedule 2 General rules for the interpretation of Schedule 3"@en-AU ;
    skos:narrower C2004A04997:56 ;
    skos:prefLabel "Item I60"@en-AU ;
    dcat:accessURL "https://www.legislation.gov.au/C2004A04997/2024-07-01/2024-07-01/text/1/epub/OEBPS/document_1/document_1.html#_Toc172806560"^^xsd:anyURI .

C2004A04997:61 a legcons:Item,
        skos:Concept,
        dcat:Resource ;
    rdfs:label "Item I61"@en-AU ;
    rdfs:comment "Schedule 3 Classification of goods and general and special rates of duty - GraphNodeID: I61"@en-AU ;
    skos:definition "Schedule 3 Classification of goods and general and special rates of duty"@en-AU ;
    skos:narrower C2004A04997:56 ;
    skos:prefLabel "Item I61"@en-AU ;
    dcat:accessURL "https://www.legislation.gov.au/C2004A04997/2024-07-01/2024-07-01/text/1/epub/OEBPS/document_1/document_1.html#_Toc172806561"^^xsd:anyURI .

C2004A04997:62 a legcons:Item,
        skos:Concept,
        dcat:Resource ;
    rdfs:label "Item I62"@en-AU ;
    rdfs:comment "Section ILive animals animal products - GraphNodeID: I62"@en-AU ;
    skos:definition "Section ILive animals animal products"@en-AU ;
    skos:narrower C2004A04997:56 ;
    skos:prefLabel "Item I62"@en-AU ;
    dcat:accessURL "https://www.legislation.gov.au/C2004A04997/2024-07-01/2024-07-01/text/1/epub/OEBPS/document_1/document_1.html#_Toc172806562"^^xsd:anyURI .

C2004A04997:63 a legcons:Item,
        skos:Concept,
        dcat:Resource ;
    rdfs:label "Item I63"@en-AU ;
    rdfs:comment "Notes - GraphNodeID: I63"@en-AU ;
    skos:definition "Notes"@en-AU ;
    skos:narrower C2004A04997:56 ;
    skos:prefLabel "Item I63"@en-AU ;
    dcat:accessURL "https://www.legislation.gov.au/C2004A04997/2024-07-01/2024-07-01/text/1/epub/OEBPS/document_1/document_1.html#_Toc172806563"^^xsd:anyURI .

C2004A04997:64 a legcons:Chapter,
        skos:Concept,
        dcat:Resource ;
    rdfs:label "Chapter C64"@en-AU ;
    rdfs:comment "Chapter 1 Live animals - GraphNodeID: C64"@en-AU ;
    skos:definition "Chapter 1 Live animals"@en-AU ;
    skos:narrower C2004A04997:1 ;
    skos:prefLabel "Chapter C64"@en-AU ;
    dcat:accessURL "https://www.legislation.gov.au/C2004A04997/2024-07-01/2024-07-01/text/1/epub/OEBPS/document_1/document_1.html#_Toc172806564"^^xsd:anyURI .

C2004A04997:65 a legcons:Item,
        skos:Concept,
        dcat:Resource ;
    rdfs:label "Item I65"@en-AU ;
    rdfs:comment "Note - GraphNodeID: I65"@en-AU ;
    skos:definition "Note"@en-AU ;
    skos:narrower C2004A04997:56 ;
    skos:prefLabel "Item I65"@en-AU ;
    dcat:accessURL "https://www.legislation.gov.au/C2004A04997/2024-07-01/2024-07-01/text/1/epub/OEBPS/document_1/document_1.html#_Toc172806565"^^xsd:anyURI .

C2004A04997:66 a legcons:Chapter,
        skos:Concept,
        dcat:Resource ;
    rdfs:label "Chapter C66"@en-AU ;
    rdfs:comment "Chapter 2 Meat and edible meat offal - GraphNodeID: C66"@en-AU ;
    skos:definition "Chapter 2 Meat and edible meat offal"@en-AU ;
    skos:narrower C2004A04997:1 ;
    skos:prefLabel "Chapter C66"@en-AU ;
    dcat:accessURL "https://www.legislation.gov.au/C2004A04997/2024-07-01/2024-07-01/text/1/epub/OEBPS/document_1/document_1.html#_Toc172806566"^^xsd:anyURI .

C2004A04997:67 a legcons:Item,
        skos:Concept,
        dcat:Resource ;
    rdfs:label "Item I67"@en-AU ;
    rdfs:comment "Note - GraphNodeID: I67"@en-AU ;
    skos:definition "Note"@en-AU ;
    skos:narrower C2004A04997:56 ;
    skos:prefLabel "Item I67"@en-AU ;
    dcat:accessURL "https://www.legislation.gov.au/C2004A04997/2024-07-01/2024-07-01/text/1/epub/OEBPS/document_1/document_1.html#_Toc172806567"^^xsd:anyURI .

C2004A04997:68 a legcons:Chapter,
        skos:Concept,
        dcat:Resource ;
    rdfs:label "Chapter C68"@en-AU ;
    rdfs:comment "Chapter 3 Fish and crustaceans molluscs and other aquatic invertebrates - GraphNodeID: C68"@en-AU ;
    skos:definition "Chapter 3 Fish and crustaceans molluscs and other aquatic invertebrates"@en-AU ;
    skos:narrower C2004A04997:1 ;
    skos:prefLabel "Chapter C68"@en-AU ;
    dcat:accessURL "https://www.legislation.gov.au/C2004A04997/2024-07-01/2024-07-01/text/1/epub/OEBPS/document_1/document_1.html#_Toc172806568"^^xsd:anyURI .

C2004A04997:69 a legcons:Item,
        skos:Concept,
        dcat:Resource ;
    rdfs:label "Item I69"@en-AU ;
    rdfs:comment "Notes - GraphNodeID: I69"@en-AU ;
    skos:definition "Notes"@en-AU ;
    skos:narrower C2004A04997:56 ;
    skos:prefLabel "Item I69"@en-AU ;
    dcat:accessURL "https://www.legislation.gov.au/C2004A04997/2024-07-01/2024-07-01/text/1/epub/OEBPS/document_1/document_1.html#_Toc172806569"^^xsd:anyURI .

C2004A04997:7 a legcons:Item,
        skos:Concept,
        dcat:Resource ;
    rdfs:label "Item I7"@en-AU ;
    rdfs:comment "4  Headings in Schedule 3 - GraphNodeID: I7"@en-AU ;
    skos:definition "4  Headings in Schedule 3"@en-AU ;
    skos:narrower C2004A04997:2 ;
    skos:prefLabel "Item I7"@en-AU ;
    dcat:accessURL "https://www.legislation.gov.au/C2004A04997/2024-07-01/2024-07-01/text/1/epub/OEBPS/document_1/document_1.html#_Toc172806507"^^xsd:anyURI .

C2004A04997:70 a legcons:Chapter,
        skos:Concept,
        dcat:Resource ;
    rdfs:label "Chapter C70"@en-AU ;
    rdfs:comment "Chapter 4 Dairy produce birds eggs natural honey edible products of animal origin not elsewhere specified or included - GraphNodeID: C70"@en-AU ;
    skos:definition "Chapter 4 Dairy produce birds eggs natural honey edible products of animal origin not elsewhere specified or included"@en-AU ;
    skos:narrower C2004A04997:1 ;
    skos:prefLabel "Chapter C70"@en-AU ;
    dcat:accessURL "https://www.legislation.gov.au/C2004A04997/2024-07-01/2024-07-01/text/1/epub/OEBPS/document_1/document_1.html#_Toc172806570"^^xsd:anyURI .

C2004A04997:71 a legcons:Item,
        skos:Concept,
        dcat:Resource ;
    rdfs:label "Item I71"@en-AU ;
    rdfs:comment "Notes - GraphNodeID: I71"@en-AU ;
    skos:definition "Notes"@en-AU ;
    skos:narrower C2004A04997:56 ;
    skos:prefLabel "Item I71"@en-AU ;
    dcat:accessURL "https://www.legislation.gov.au/C2004A04997/2024-07-01/2024-07-01/text/1/epub/OEBPS/document_1/document_1.html#_Toc172806571"^^xsd:anyURI .

C2004A04997:72 a legcons:Item,
        skos:Concept,
        dcat:Resource ;
    rdfs:label "Item I72"@en-AU ;
    rdfs:comment "Subheading Notes - GraphNodeID: I72"@en-AU ;
    skos:definition "Subheading Notes"@en-AU ;
    skos:narrower C2004A04997:56 ;
    skos:prefLabel "Item I72"@en-AU ;
    dcat:accessURL "https://www.legislation.gov.au/C2004A04997/2024-07-01/2024-07-01/text/1/epub/OEBPS/document_1/document_1.html#_Toc172806572"^^xsd:anyURI .

C2004A04997:73 a legcons:Chapter,
        skos:Concept,
        dcat:Resource ;
    rdfs:label "Chapter C73"@en-AU ;
    rdfs:comment "Chapter 5 Products of animal origin not elsewhere specified or included - GraphNodeID: C73"@en-AU ;
    skos:definition "Chapter 5 Products of animal origin not elsewhere specified or included"@en-AU ;
    skos:narrower C2004A04997:1 ;
    skos:prefLabel "Chapter C73"@en-AU ;
    dcat:accessURL "https://www.legislation.gov.au/C2004A04997/2024-07-01/2024-07-01/text/1/epub/OEBPS/document_1/document_1.html#_Toc172806573"^^xsd:anyURI .

C2004A04997:74 a legcons:Item,
        skos:Concept,
        dcat:Resource ;
    rdfs:label "Item I74"@en-AU ;
    rdfs:comment "Notes - GraphNodeID: I74"@en-AU ;
    skos:definition "Notes"@en-AU ;
    skos:narrower C2004A04997:56 ;
    skos:prefLabel "Item I74"@en-AU ;
    dcat:accessURL "https://www.legislation.gov.au/C2004A04997/2024-07-01/2024-07-01/text/1/epub/OEBPS/document_1/document_1.html#_Toc172806574"^^xsd:anyURI .

C2004A04997:75 a legcons:Item,
        skos:Concept,
        dcat:Resource ;
    rdfs:label "Item I75"@en-AU ;
    rdfs:comment "Section IIVegetable products - GraphNodeID: I75"@en-AU ;
    skos:definition "Section IIVegetable products"@en-AU ;
    skos:narrower C2004A04997:56 ;
    skos:prefLabel "Item I75"@en-AU ;
    dcat:accessURL "https://www.legislation.gov.au/C2004A04997/2024-07-01/2024-07-01/text/1/epub/OEBPS/document_1/document_1.html#_Toc172806575"^^xsd:anyURI .

C2004A04997:76 a legcons:Item,
        skos:Concept,
        dcat:Resource ;
    rdfs:label "Item I76"@en-AU ;
    rdfs:comment "Note - GraphNodeID: I76"@en-AU ;
    skos:definition "Note"@en-AU ;
    skos:narrower C2004A04997:56 ;
    skos:prefLabel "Item I76"@en-AU ;
    dcat:accessURL "https://www.legislation.gov.au/C2004A04997/2024-07-01/2024-07-01/text/1/epub/OEBPS/document_1/document_1.html#_Toc172806576"^^xsd:anyURI .

C2004A04997:77 a legcons:Chapter,
        skos:Concept,
        dcat:Resource ;
    rdfs:label "Chapter C77"@en-AU ;
    rdfs:comment "Chapter 6 Live trees and other plants bulbs roots and the like cut flowers and ornamental foliage - GraphNodeID: C77"@en-AU ;
    skos:definition "Chapter 6 Live trees and other plants bulbs roots and the like cut flowers and ornamental foliage"@en-AU ;
    skos:narrower C2004A04997:1 ;
    skos:prefLabel "Chapter C77"@en-AU ;
    dcat:accessURL "https://www.legislation.gov.au/C2004A04997/2024-07-01/2024-07-01/text/1/epub/OEBPS/document_1/document_1.html#_Toc172806577"^^xsd:anyURI .

C2004A04997:78 a legcons:Item,
        skos:Concept,
        dcat:Resource ;
    rdfs:label "Item I78"@en-AU ;
    rdfs:comment "Notes - GraphNodeID: I78"@en-AU ;
    skos:definition "Notes"@en-AU ;
    skos:narrower C2004A04997:56 ;
    skos:prefLabel "Item I78"@en-AU ;
    dcat:accessURL "https://www.legislation.gov.au/C2004A04997/2024-07-01/2024-07-01/text/1/epub/OEBPS/document_1/document_1.html#_Toc172806578"^^xsd:anyURI .

C2004A04997:79 a legcons:Chapter,
        skos:Concept,
        dcat:Resource ;
    rdfs:label "Chapter C79"@en-AU ;
    rdfs:comment "Chapter 7 Edible vegetables and certain roots and tubers - GraphNodeID: C79"@en-AU ;
    skos:definition "Chapter 7 Edible vegetables and certain roots and tubers"@en-AU ;
    skos:narrower C2004A04997:1 ;
    skos:prefLabel "Chapter C79"@en-AU ;
    dcat:accessURL "https://www.legislation.gov.au/C2004A04997/2024-07-01/2024-07-01/text/1/epub/OEBPS/document_1/document_1.html#_Toc172806579"^^xsd:anyURI .

C2004A04997:8 a legcons:Item,
        skos:Concept,
        dcat:Resource ;
    rdfs:label "Item I8"@en-AU ;
    rdfs:comment "5  Items in Schedule 4 - GraphNodeID: I8"@en-AU ;
    skos:definition "5  Items in Schedule 4"@en-AU ;
    skos:narrower C2004A04997:2 ;
    skos:prefLabel "Item I8"@en-AU ;
    dcat:accessURL "https://www.legislation.gov.au/C2004A04997/2024-07-01/2024-07-01/text/1/epub/OEBPS/document_1/document_1.html#_Toc172806508"^^xsd:anyURI .

C2004A04997:80 a legcons:Item,
        skos:Concept,
        dcat:Resource ;
    rdfs:label "Item I80"@en-AU ;
    rdfs:comment "Notes - GraphNodeID: I80"@en-AU ;
    skos:definition "Notes"@en-AU ;
    skos:narrower C2004A04997:56 ;
    skos:prefLabel "Item I80"@en-AU ;
    dcat:accessURL "https://www.legislation.gov.au/C2004A04997/2024-07-01/2024-07-01/text/1/epub/OEBPS/document_1/document_1.html#_Toc172806580"^^xsd:anyURI .

C2004A04997:81 a legcons:Chapter,
        skos:Concept,
        dcat:Resource ;
    rdfs:label "Chapter C81"@en-AU ;
    rdfs:comment "Chapter 8 Edible fruit and nuts peel of citrus fruit or melons - GraphNodeID: C81"@en-AU ;
    skos:definition "Chapter 8 Edible fruit and nuts peel of citrus fruit or melons"@en-AU ;
    skos:narrower C2004A04997:1 ;
    skos:prefLabel "Chapter C81"@en-AU ;
    dcat:accessURL "https://www.legislation.gov.au/C2004A04997/2024-07-01/2024-07-01/text/1/epub/OEBPS/document_1/document_1.html#_Toc172806581"^^xsd:anyURI .

C2004A04997:82 a legcons:Item,
        skos:Concept,
        dcat:Resource ;
    rdfs:label "Item I82"@en-AU ;
    rdfs:comment "Notes - GraphNodeID: I82"@en-AU ;
    skos:definition "Notes"@en-AU ;
    skos:narrower C2004A04997:56 ;
    skos:prefLabel "Item I82"@en-AU ;
    dcat:accessURL "https://www.legislation.gov.au/C2004A04997/2024-07-01/2024-07-01/text/1/epub/OEBPS/document_1/document_1.html#_Toc172806582"^^xsd:anyURI .

C2004A04997:83 a legcons:Chapter,
        skos:Concept,
        dcat:Resource ;
    rdfs:label "Chapter C83"@en-AU ;
    rdfs:comment "Chapter 9 Coffee tea mate and spices - GraphNodeID: C83"@en-AU ;
    skos:definition "Chapter 9 Coffee tea mate and spices"@en-AU ;
    skos:narrower C2004A04997:1 ;
    skos:prefLabel "Chapter C83"@en-AU ;
    dcat:accessURL "https://www.legislation.gov.au/C2004A04997/2024-07-01/2024-07-01/text/1/epub/OEBPS/document_1/document_1.html#_Toc172806583"^^xsd:anyURI .

C2004A04997:84 a legcons:Item,
        skos:Concept,
        dcat:Resource ;
    rdfs:label "Item I84"@en-AU ;
    rdfs:comment "Notes - GraphNodeID: I84"@en-AU ;
    skos:definition "Notes"@en-AU ;
    skos:narrower C2004A04997:56 ;
    skos:prefLabel "Item I84"@en-AU ;
    dcat:accessURL "https://www.legislation.gov.au/C2004A04997/2024-07-01/2024-07-01/text/1/epub/OEBPS/document_1/document_1.html#_Toc172806584"^^xsd:anyURI .

C2004A04997:85 a legcons:Chapter,
        skos:Concept,
        dcat:Resource ;
    rdfs:label "Chapter C85"@en-AU ;
    rdfs:comment "Chapter 10 Cereals - GraphNodeID: C85"@en-AU ;
    skos:definition "Chapter 10 Cereals"@en-AU ;
    skos:narrower C2004A04997:1 ;
    skos:prefLabel "Chapter C85"@en-AU ;
    dcat:accessURL "https://www.legislation.gov.au/C2004A04997/2024-07-01/2024-07-01/text/1/epub/OEBPS/document_1/document_1.html#_Toc172806585"^^xsd:anyURI .

C2004A04997:86 a legcons:Item,
        skos:Concept,
        dcat:Resource ;
    rdfs:label "Item I86"@en-AU ;
    rdfs:comment "Notes - GraphNodeID: I86"@en-AU ;
    skos:definition "Notes"@en-AU ;
    skos:narrower C2004A04997:56 ;
    skos:prefLabel "Item I86"@en-AU ;
    dcat:accessURL "https://www.legislation.gov.au/C2004A04997/2024-07-01/2024-07-01/text/1/epub/OEBPS/document_1/document_1.html#_Toc172806586"^^xsd:anyURI .

C2004A04997:87 a legcons:Item,
        skos:Concept,
        dcat:Resource ;
    rdfs:label "Item I87"@en-AU ;
    rdfs:comment "Subheading Note - GraphNodeID: I87"@en-AU ;
    skos:definition "Subheading Note"@en-AU ;
    skos:narrower C2004A04997:56 ;
    skos:prefLabel "Item I87"@en-AU ;
    dcat:accessURL "https://www.legislation.gov.au/C2004A04997/2024-07-01/2024-07-01/text/1/epub/OEBPS/document_1/document_1.html#_Toc172806587"^^xsd:anyURI .

C2004A04997:88 a legcons:Chapter,
        skos:Concept,
        dcat:Resource ;
    rdfs:label "Chapter C88"@en-AU ;
    rdfs:comment "Chapter 11 Products of the milling industry malt starches inulin wheat gluten - GraphNodeID: C88"@en-AU ;
    skos:definition "Chapter 11 Products of the milling industry malt starches inulin wheat gluten"@en-AU ;
    skos:narrower C2004A04997:1 ;
    skos:prefLabel "Chapter C88"@en-AU ;
    dcat:accessURL "https://www.legislation.gov.au/C2004A04997/2024-07-01/2024-07-01/text/1/epub/OEBPS/document_1/document_1.html#_Toc172806588"^^xsd:anyURI .

C2004A04997:89 a legcons:Item,
        skos:Concept,
        dcat:Resource ;
    rdfs:label "Item I89"@en-AU ;
    rdfs:comment "Notes - GraphNodeID: I89"@en-AU ;
    skos:definition "Notes"@en-AU ;
    skos:narrower C2004A04997:56 ;
    skos:prefLabel "Item I89"@en-AU ;
    dcat:accessURL "https://www.legislation.gov.au/C2004A04997/2024-07-01/2024-07-01/text/1/epub/OEBPS/document_1/document_1.html#_Toc172806589"^^xsd:anyURI .

C2004A04997:9 a legcons:Item,
        skos:Concept,
        dcat:Resource ;
    rdfs:label "Item I9"@en-AU ;
    rdfs:comment "6  Tariff classification - GraphNodeID: I9"@en-AU ;
    skos:definition "6  Tariff classification"@en-AU ;
    skos:narrower C2004A04997:2 ;
    skos:prefLabel "Item I9"@en-AU ;
    dcat:accessURL "https://www.legislation.gov.au/C2004A04997/2024-07-01/2024-07-01/text/1/epub/OEBPS/document_1/document_1.html#_Toc172806509"^^xsd:anyURI .

C2004A04997:90 a legcons:Chapter,
        skos:Concept,
        dcat:Resource ;
    rdfs:label "Chapter C90"@en-AU ;
    rdfs:comment "Chapter 12 Oil seeds and oleaginous fruits miscellaneous grains seeds and fruit industrial or medicinal plants straw and fodder - GraphNodeID: C90"@en-AU ;
    skos:definition "Chapter 12 Oil seeds and oleaginous fruits miscellaneous grains seeds and fruit industrial or medicinal plants straw and fodder"@en-AU ;
    skos:narrower C2004A04997:1 ;
    skos:prefLabel "Chapter C90"@en-AU ;
    dcat:accessURL "https://www.legislation.gov.au/C2004A04997/2024-07-01/2024-07-01/text/1/epub/OEBPS/document_1/document_1.html#_Toc172806590"^^xsd:anyURI .

C2004A04997:91 a legcons:Item,
        skos:Concept,
        dcat:Resource ;
    rdfs:label "Item I91"@en-AU ;
    rdfs:comment "Notes - GraphNodeID: I91"@en-AU ;
    skos:definition "Notes"@en-AU ;
    skos:narrower C2004A04997:56 ;
    skos:prefLabel "Item I91"@en-AU ;
    dcat:accessURL "https://www.legislation.gov.au/C2004A04997/2024-07-01/2024-07-01/text/1/epub/OEBPS/document_1/document_1.html#_Toc172806591"^^xsd:anyURI .

C2004A04997:92 a legcons:Item,
        skos:Concept,
        dcat:Resource ;
    rdfs:label "Item I92"@en-AU ;
    rdfs:comment "Subheading Note - GraphNodeID: I92"@en-AU ;
    skos:definition "Subheading Note"@en-AU ;
    skos:narrower C2004A04997:56 ;
    skos:prefLabel "Item I92"@en-AU ;
    dcat:accessURL "https://www.legislation.gov.au/C2004A04997/2024-07-01/2024-07-01/text/1/epub/OEBPS/document_1/document_1.html#_Toc172806592"^^xsd:anyURI .

C2004A04997:93 a legcons:Chapter,
        skos:Concept,
        dcat:Resource ;
    rdfs:label "Chapter C93"@en-AU ;
    rdfs:comment "Chapter 13 Lac gums resins and other vegetable saps and extracts - GraphNodeID: C93"@en-AU ;
    skos:definition "Chapter 13 Lac gums resins and other vegetable saps and extracts"@en-AU ;
    skos:narrower C2004A04997:1 ;
    skos:prefLabel "Chapter C93"@en-AU ;
    dcat:accessURL "https://www.legislation.gov.au/C2004A04997/2024-07-01/2024-07-01/text/1/epub/OEBPS/document_1/document_1.html#_Toc172806593"^^xsd:anyURI .

C2004A04997:94 a legcons:Item,
        skos:Concept,
        dcat:Resource ;
    rdfs:label "Item I94"@en-AU ;
    rdfs:comment "Note - GraphNodeID: I94"@en-AU ;
    skos:definition "Note"@en-AU ;
    skos:narrower C2004A04997:56 ;
    skos:prefLabel "Item I94"@en-AU ;
    dcat:accessURL "https://www.legislation.gov.au/C2004A04997/2024-07-01/2024-07-01/text/1/epub/OEBPS/document_1/document_1.html#_Toc172806594"^^xsd:anyURI .

C2004A04997:95 a legcons:Chapter,
        skos:Concept,
        dcat:Resource ;
    rdfs:label "Chapter C95"@en-AU ;
    rdfs:comment "Chapter 14 Vegetable plaiting materials vegetable products not elsewhere specified or included - GraphNodeID: C95"@en-AU ;
    skos:definition "Chapter 14 Vegetable plaiting materials vegetable products not elsewhere specified or included"@en-AU ;
    skos:narrower C2004A04997:1 ;
    skos:prefLabel "Chapter C95"@en-AU ;
    dcat:accessURL "https://www.legislation.gov.au/C2004A04997/2024-07-01/2024-07-01/text/1/epub/OEBPS/document_1/document_1.html#_Toc172806595"^^xsd:anyURI .

C2004A04997:96 a legcons:Item,
        skos:Concept,
        dcat:Resource ;
    rdfs:label "Item I96"@en-AU ;
    rdfs:comment "Notes - GraphNodeID: I96"@en-AU ;
    skos:definition "Notes"@en-AU ;
    skos:narrower C2004A04997:56 ;
    skos:prefLabel "Item I96"@en-AU ;
    dcat:accessURL "https://www.legislation.gov.au/C2004A04997/2024-07-01/2024-07-01/text/1/epub/OEBPS/document_1/document_1.html#_Toc172806596"^^xsd:anyURI .

C2004A04997:97 a legcons:Item,
        skos:Concept,
        dcat:Resource ;
    rdfs:label "Item I97"@en-AU ;
    rdfs:comment "Section IIIAnimal vegetable or microbial fats and oils and their cleavage products prepared edible fats animal or vegetable waxes - GraphNodeID: I97"@en-AU ;
    skos:definition "Section IIIAnimal vegetable or microbial fats and oils and their cleavage products prepared edible fats animal or vegetable waxes"@en-AU ;
    skos:narrower C2004A04997:56 ;
    skos:prefLabel "Item I97"@en-AU ;
    dcat:accessURL "https://www.legislation.gov.au/C2004A04997/2024-07-01/2024-07-01/text/1/epub/OEBPS/document_1/document_1.html#_Toc172806597"^^xsd:anyURI .

C2004A04997:98 a legcons:Chapter,
        skos:Concept,
        dcat:Resource ;
    rdfs:label "Chapter C98"@en-AU ;
    rdfs:comment "Chapter 15 Animal vegetable or microbial fats and oils and their cleavage products prepared edible fats animal or vegetable waxes - GraphNodeID: C98"@en-AU ;
    skos:definition "Chapter 15 Animal vegetable or microbial fats and oils and their cleavage products prepared edible fats animal or vegetable waxes"@en-AU ;
    skos:narrower C2004A04997:1 ;
    skos:prefLabel "Chapter C98"@en-AU ;
    dcat:accessURL "https://www.legislation.gov.au/C2004A04997/2024-07-01/2024-07-01/text/1/epub/OEBPS/document_1/document_1.html#_Toc172806598"^^xsd:anyURI .

C2004A04997:99 a legcons:Item,
        skos:Concept,
        dcat:Resource ;
    rdfs:label "Item I99"@en-AU ;
    rdfs:comment "Notes - GraphNodeID: I99"@en-AU ;
    skos:definition "Notes"@en-AU ;
    skos:narrower C2004A04997:56 ;
    skos:prefLabel "Item I99"@en-AU ;
    dcat:accessURL "https://www.legislation.gov.au/C2004A04997/2024-07-01/2024-07-01/text/1/epub/OEBPS/document_1/document_1.html#_Toc172806599"^^xsd:anyURI .

C2004A04997:385 a legcons:Chapter,
        skos:Concept,
        dcat:Resource ;
    rdfs:label "Chapter C385"@en-AU ;
    rdfs:comment "Chapter 97 Works of art collectors pieces and antiques - GraphNodeID: C385"@en-AU ;
    skos:broader C2004A04997:408 ;
    skos:definition "Chapter 97 Works of art collectors pieces and antiques"@en-AU ;
    skos:narrower C2004A04997:317 ;
    skos:prefLabel "Chapter C385"@en-AU ;
    dcat:accessURL "https://www.legislation.gov.au/C2004A04997/2024-07-01/2024-07-01/text/1/epub/OEBPS/document_5/document_5.html#_Toc171753227"^^xsd:anyURI .

C2004A04997:408 a legcons:Part,
        skos:Concept,
        dcat:Resource ;
    rdfs:label "Part P408"@en-AU ;
    rdfs:comment "Endnotes - GraphNodeID: P408"@en-AU ;
    skos:broader C2004A04997:409,
        C2004A04997:410,
        C2004A04997:411,
        C2004A04997:412 ;
    skos:definition "Endnotes"@en-AU ;
    skos:narrower C2004A04997:385 ;
    skos:prefLabel "Part P408"@en-AU ;
    dcat:accessURL "https://www.legislation.gov.au/C2004A04997/2024-07-01/2024-07-01/text/1/epub/OEBPS/document_7/document_7.html#_Toc171755738"^^xsd:anyURI .

C2004A04997:259 a legcons:Volume,
        skos:Concept,
        dcat:Resource ;
    rdfs:label "Volume V259"@en-AU ;
    rdfs:comment "Volume 4 - GraphNodeID: V259"@en-AU ;
    skos:broader C2004A04997:262,
        C2004A04997:265,
        C2004A04997:268,
        C2004A04997:271,
        C2004A04997:278,
        C2004A04997:281,
        C2004A04997:283,
        C2004A04997:285,
        C2004A04997:288,
        C2004A04997:290,
        C2004A04997:294,
        C2004A04997:298,
        C2004A04997:306,
        C2004A04997:314 ;
    skos:definition "Volume 4"@en-AU ;
    skos:prefLabel "Volume V259"@en-AU ;
    dcat:accessURL "https://www.legislation.gov.au/C2004A04997/2024-07-01/2024-07-01/text/1/epub/OEBPS/document_4/document_4.html"^^xsd:anyURI .

C2004A04997:1 a legcons:Volume,
        skos:Concept,
        dcat:Resource ;
    rdfs:label "Volume V1"@en-AU ;
    rdfs:comment "Volume 1 - GraphNodeID: V1"@en-AU ;
    skos:broader C2004A04997:2,
        C2004A04997:36,
        C2004A04997:56,
        C2004A04997:64,
        C2004A04997:66,
        C2004A04997:68,
        C2004A04997:70,
        C2004A04997:73,
        C2004A04997:77,
        C2004A04997:79,
        C2004A04997:81,
        C2004A04997:83,
        C2004A04997:85,
        C2004A04997:88,
        C2004A04997:90,
        C2004A04997:93,
        C2004A04997:95,
        C2004A04997:98 ;
    skos:definition "Volume 1"@en-AU ;
    skos:prefLabel "Volume V1"@en-AU ;
    dcat:accessURL "https://www.legislation.gov.au/C2004A04997/2024-07-01/2024-07-01/text/1/epub/OEBPS/document_1/document_1.html"^^xsd:anyURI .

C2004A04997:36 a legcons:Part,
        skos:Concept,
        dcat:Resource ;
    rdfs:label "Part P36"@en-AU ;
    rdfs:comment "Part 2 Duties of Customs - GraphNodeID: P36"@en-AU ;
    skos:broader C2004A04997:37,
        C2004A04997:38,
        C2004A04997:39,
        C2004A04997:40,
        C2004A04997:41,
        C2004A04997:42,
        C2004A04997:43,
        C2004A04997:44,
        C2004A04997:45,
        C2004A04997:46,
        C2004A04997:47,
        C2004A04997:48,
        C2004A04997:49,
        C2004A04997:50,
        C2004A04997:51,
        C2004A04997:52,
        C2004A04997:53,
        C2004A04997:54,
        C2004A04997:55 ;
    skos:definition "Part 2 Duties of Customs"@en-AU ;
    skos:narrower C2004A04997:1 ;
    skos:prefLabel "Part P36"@en-AU ;
    dcat:accessURL "https://www.legislation.gov.au/C2004A04997/2024-07-01/2024-07-01/text/1/epub/OEBPS/document_1/document_1.html#_Toc172806536"^^xsd:anyURI .

C2004A04997:197 a legcons:Volume,
        skos:Concept,
        dcat:Resource ;
    rdfs:label "Volume V197"@en-AU ;
    rdfs:comment "Volume 3 - GraphNodeID: V197"@en-AU ;
    skos:broader C2004A04997:202,
        C2004A04997:208,
        C2004A04997:211,
        C2004A04997:213,
        C2004A04997:215,
        C2004A04997:218,
        C2004A04997:222,
        C2004A04997:224,
        C2004A04997:227,
        C2004A04997:229,
        C2004A04997:233,
        C2004A04997:239,
        C2004A04997:240,
        C2004A04997:242,
        C2004A04997:244,
        C2004A04997:245,
        C2004A04997:247,
        C2004A04997:249,
        C2004A04997:251,
        C2004A04997:254,
        C2004A04997:257 ;
    skos:definition "Volume 3"@en-AU ;
    skos:prefLabel "Volume V197"@en-AU ;
    dcat:accessURL "https://www.legislation.gov.au/C2004A04997/2024-07-01/2024-07-01/text/1/epub/OEBPS/document_3/document_3.html"^^xsd:anyURI .

C2004A04997:102 a legcons:Volume,
        skos:Concept,
        dcat:Resource ;
    rdfs:label "Volume V102"@en-AU ;
    rdfs:comment "Volume 2 - GraphNodeID: V102"@en-AU ;
    skos:broader C2004A04997:107,
        C2004A04997:110,
        C2004A04997:113,
        C2004A04997:115,
        C2004A04997:118,
        C2004A04997:122,
        C2004A04997:125,
        C2004A04997:129,
        C2004A04997:132,
        C2004A04997:137,
        C2004A04997:139,
        C2004A04997:142,
        C2004A04997:148,
        C2004A04997:158,
        C2004A04997:175,
        C2004A04997:179,
        C2004A04997:181,
        C2004A04997:183,
        C2004A04997:185,
        C2004A04997:187,
        C2004A04997:189,
        C2004A04997:191,
        C2004A04997:193 ;
    skos:definition "Volume 2"@en-AU ;
    skos:prefLabel "Volume V102"@en-AU ;
    dcat:accessURL "https://www.legislation.gov.au/C2004A04997/2024-07-01/2024-07-01/text/1/epub/OEBPS/document_2/document_2.html"^^xsd:anyURI .

C2004A04997:317 a legcons:Volume,
        skos:Concept,
        dcat:Resource ;
    rdfs:label "Volume V317"@en-AU ;
    rdfs:comment "Volume 5 - GraphNodeID: V317"@en-AU ;
    skos:broader C2004A04997:320,
        C2004A04997:323,
        C2004A04997:325,
        C2004A04997:328,
        C2004A04997:330,
        C2004A04997:332,
        C2004A04997:334,
        C2004A04997:335,
        C2004A04997:337,
        C2004A04997:343,
        C2004A04997:347,
        C2004A04997:353,
        C2004A04997:355,
        C2004A04997:359,
        C2004A04997:362,
        C2004A04997:365,
        C2004A04997:368,
        C2004A04997:370,
        C2004A04997:373,
        C2004A04997:376,
        C2004A04997:379,
        C2004A04997:382,
        C2004A04997:385 ;
    skos:definition "Volume 5"@en-AU ;
    skos:prefLabel "Volume V317"@en-AU ;
    dcat:accessURL "https://www.legislation.gov.au/C2004A04997/2024-07-01/2024-07-01/text/1/epub/OEBPS/document_5/document_5.html"^^xsd:anyURI .

C2004A04997:2 a legcons:Part,
        skos:Concept,
        dcat:Resource ;
    rdfs:label "Part P2"@en-AU ;
    rdfs:comment "Part 1 Preliminary - GraphNodeID: P2"@en-AU ;
    skos:broader C2004A04997:10,
        C2004A04997:11,
        C2004A04997:12,
        C2004A04997:13,
        C2004A04997:14,
        C2004A04997:15,
        C2004A04997:16,
        C2004A04997:17,
        C2004A04997:18,
        C2004A04997:19,
        C2004A04997:20,
        C2004A04997:21,
        C2004A04997:22,
        C2004A04997:23,
        C2004A04997:24,
        C2004A04997:25,
        C2004A04997:26,
        C2004A04997:27,
        C2004A04997:28,
        C2004A04997:29,
        C2004A04997:3,
        C2004A04997:30,
        C2004A04997:31,
        C2004A04997:32,
        C2004A04997:33,
        C2004A04997:34,
        C2004A04997:35,
        C2004A04997:4,
        C2004A04997:5,
        C2004A04997:6,
        C2004A04997:7,
        C2004A04997:8,
        C2004A04997:9 ;
    skos:definition "Part 1 Preliminary"@en-AU ;
    skos:narrower C2004A04997:1 ;
    skos:prefLabel "Part P2"@en-AU ;
    dcat:accessURL "https://www.legislation.gov.au/C2004A04997/2024-07-01/2024-07-01/text/1/epub/OEBPS/document_1/document_1.html#_Toc172806502"^^xsd:anyURI .

C2004A04997:56 a legcons:Part,
        skos:Concept,
        dcat:Resource ;
    rdfs:label "Part P56"@en-AU ;
    rdfs:comment "Part 3 Miscellaneous - GraphNodeID: P56"@en-AU ;
    skos:broader C2004A04997:100,
        C2004A04997:101,
        C2004A04997:103,
        C2004A04997:104,
        C2004A04997:105,
        C2004A04997:106,
        C2004A04997:108,
        C2004A04997:109,
        C2004A04997:111,
        C2004A04997:112,
        C2004A04997:114,
        C2004A04997:116,
        C2004A04997:117,
        C2004A04997:119,
        C2004A04997:120,
        C2004A04997:121,
        C2004A04997:123,
        C2004A04997:124,
        C2004A04997:126,
        C2004A04997:127,
        C2004A04997:128,
        C2004A04997:130,
        C2004A04997:131,
        C2004A04997:133,
        C2004A04997:134,
        C2004A04997:135,
        C2004A04997:136,
        C2004A04997:138,
        C2004A04997:140,
        C2004A04997:141,
        C2004A04997:143,
        C2004A04997:144,
        C2004A04997:145,
        C2004A04997:146,
        C2004A04997:147,
        C2004A04997:149,
        C2004A04997:150,
        C2004A04997:151,
        C2004A04997:152,
        C2004A04997:153,
        C2004A04997:154,
        C2004A04997:155,
        C2004A04997:156,
        C2004A04997:157,
        C2004A04997:159,
        C2004A04997:160,
        C2004A04997:161,
        C2004A04997:162,
        C2004A04997:163,
        C2004A04997:164,
        C2004A04997:165,
        C2004A04997:166,
        C2004A04997:167,
        C2004A04997:168,
        C2004A04997:169,
        C2004A04997:170,
        C2004A04997:171,
        C2004A04997:172,
        C2004A04997:173,
        C2004A04997:174,
        C2004A04997:176,
        C2004A04997:177,
        C2004A04997:178,
        C2004A04997:180,
        C2004A04997:182,
        C2004A04997:184,
        C2004A04997:186,
        C2004A04997:188,
        C2004A04997:190,
        C2004A04997:192,
        C2004A04997:194,
        C2004A04997:195,
        C2004A04997:196,
        C2004A04997:198,
        C2004A04997:199,
        C2004A04997:200,
        C2004A04997:201,
        C2004A04997:203,
        C2004A04997:204,
        C2004A04997:205,
        C2004A04997:206,
        C2004A04997:207,
        C2004A04997:209,
        C2004A04997:210,
        C2004A04997:212,
        C2004A04997:214,
        C2004A04997:216,
        C2004A04997:217,
        C2004A04997:219,
        C2004A04997:220,
        C2004A04997:221,
        C2004A04997:223,
        C2004A04997:225,
        C2004A04997:226,
        C2004A04997:228,
        C2004A04997:230,
        C2004A04997:231,
        C2004A04997:232,
        C2004A04997:234,
        C2004A04997:235,
        C2004A04997:236,
        C2004A04997:237,
        C2004A04997:238,
        C2004A04997:241,
        C2004A04997:243,
        C2004A04997:246,
        C2004A04997:248,
        C2004A04997:250,
        C2004A04997:252,
        C2004A04997:253,
        C2004A04997:255,
        C2004A04997:256,
        C2004A04997:258,
        C2004A04997:260,
        C2004A04997:261,
        C2004A04997:263,
        C2004A04997:264,
        C2004A04997:266,
        C2004A04997:267,
        C2004A04997:269,
        C2004A04997:270,
        C2004A04997:272,
        C2004A04997:273,
        C2004A04997:274,
        C2004A04997:275,
        C2004A04997:276,
        C2004A04997:277,
        C2004A04997:279,
        C2004A04997:280,
        C2004A04997:282,
        C2004A04997:284,
        C2004A04997:286,
        C2004A04997:287,
        C2004A04997:289,
        C2004A04997:291,
        C2004A04997:292,
        C2004A04997:293,
        C2004A04997:295,
        C2004A04997:296,
        C2004A04997:297,
        C2004A04997:299,
        C2004A04997:300,
        C2004A04997:301,
        C2004A04997:302,
        C2004A04997:303,
        C2004A04997:304,
        C2004A04997:305,
        C2004A04997:307,
        C2004A04997:308,
        C2004A04997:309,
        C2004A04997:310,
        C2004A04997:311,
        C2004A04997:312,
        C2004A04997:313,
        C2004A04997:315,
        C2004A04997:316,
        C2004A04997:318,
        C2004A04997:319,
        C2004A04997:321,
        C2004A04997:322,
        C2004A04997:324,
        C2004A04997:326,
        C2004A04997:327,
        C2004A04997:329,
        C2004A04997:331,
        C2004A04997:333,
        C2004A04997:336,
        C2004A04997:338,
        C2004A04997:339,
        C2004A04997:340,
        C2004A04997:341,
        C2004A04997:342,
        C2004A04997:344,
        C2004A04997:345,
        C2004A04997:346,
        C2004A04997:348,
        C2004A04997:349,
        C2004A04997:350,
        C2004A04997:351,
        C2004A04997:352,
        C2004A04997:354,
        C2004A04997:356,
        C2004A04997:357,
        C2004A04997:358,
        C2004A04997:360,
        C2004A04997:361,
        C2004A04997:363,
        C2004A04997:364,
        C2004A04997:366,
        C2004A04997:367,
        C2004A04997:369,
        C2004A04997:371,
        C2004A04997:372,
        C2004A04997:374,
        C2004A04997:375,
        C2004A04997:377,
        C2004A04997:378,
        C2004A04997:380,
        C2004A04997:381,
        C2004A04997:383,
        C2004A04997:384,
        C2004A04997:386,
        C2004A04997:387,
        C2004A04997:389,
        C2004A04997:390,
        C2004A04997:391,
        C2004A04997:392,
        C2004A04997:393,
        C2004A04997:394,
        C2004A04997:395,
        C2004A04997:396,
        C2004A04997:397,
        C2004A04997:398,
        C2004A04997:399,
        C2004A04997:400,
        C2004A04997:401,
        C2004A04997:402,
        C2004A04997:403,
        C2004A04997:404,
        C2004A04997:405,
        C2004A04997:406,
        C2004A04997:57,
        C2004A04997:58,
        C2004A04997:59,
        C2004A04997:60,
        C2004A04997:61,
        C2004A04997:62,
        C2004A04997:63,
        C2004A04997:65,
        C2004A04997:67,
        C2004A04997:69,
        C2004A04997:71,
        C2004A04997:72,
        C2004A04997:74,
        C2004A04997:75,
        C2004A04997:76,
        C2004A04997:78,
        C2004A04997:80,
        C2004A04997:82,
        C2004A04997:84,
        C2004A04997:86,
        C2004A04997:87,
        C2004A04997:89,
        C2004A04997:91,
        C2004A04997:92,
        C2004A04997:94,
        C2004A04997:96,
        C2004A04997:97,
        C2004A04997:99 ;
    skos:definition "Part 3 Miscellaneous"@en-AU ;
    skos:narrower C2004A04997:1 ;
    skos:prefLabel "Part P56"@en-AU ;
    dcat:accessURL "https://www.legislation.gov.au/C2004A04997/2024-07-01/2024-07-01/text/1/epub/OEBPS/document_1/document_1.html#_Toc172806556"^^xsd:anyURI .

