@prefix C2004A01224: <http://example.org/au/leg/dataset/C2004A01224/> .
@prefix dcat: <http://www.w3.org/ns/dcat#> .
@prefix dct: <http://purl.org/dc/terms/> .
@prefix legcons: <http://example.org/au/leg/concepts/> .
@prefix owl: <http://www.w3.org/2002/07/owl#> .
@prefix rdfs: <http://www.w3.org/2000/01/rdf-schema#> .
@prefix schema: <https://schema.org/> .
@prefix skos: <http://www.w3.org/2004/02/skos/core#> .
@prefix xsd: <http://www.w3.org/2001/XMLSchema#> .

C2004A01224:10 a legcons:Item,
        C2004A01224:Item,
        owl:Class,
        dcat:Resource ;
    rdfs:label "Item - I10 6  Definitions of rule maker and responsible person"@en-AU ;
    dct:isPartOf C2004A01224:1 ;
    rdfs:comment "6  Definitions of rule maker and responsible person - Abrievated Graph Key: I10"@en-AU ;
    rdfs:subClassOf C2004A01224: ;
    skos:definition "6  Definitions of rule maker and responsible person"@en-AU ;
    skos:narrower C2004A01224:1 ;
    skos:prefLabel "Item I10"@en-AU ;
    dcat:accessURL <https://www.legislation.gov.au/C2004A01224/2019-02-24/2019-02-24/text/1/epub/OEBPS/document_1/document_1.html#_Toc1469130> ;
    dcat:landingPage "https://www.legislation.gov.au/C2004A01224/2019-02-24/2019-02-24/text/1/epub/OEBPS/document_1/document_1.html#_Toc1469130"^^xsd:anyURI ;
    dcat:theme legcons:Item .

C2004A01224:100 a legcons:Item,
        C2004A01224:Item,
        owl:Class,
        dcat:Resource ;
    rdfs:label "Item - I100 53  Resolution that instrument continue in force"@en-AU ;
    dct:isPartOf C2004A01224:60 ;
    rdfs:comment "53  Resolution that instrument continue in force - Abrievated Graph Key: I100"@en-AU ;
    rdfs:subClassOf C2004A01224: ;
    skos:definition "53  Resolution that instrument continue in force"@en-AU ;
    skos:narrower C2004A01224:60 ;
    skos:prefLabel "Item I100"@en-AU ;
    dcat:accessURL <https://www.legislation.gov.au/C2004A01224/2019-02-24/2019-02-24/text/1/epub/OEBPS/document_1/document_1.html#_Toc1469220> ;
    dcat:landingPage "https://www.legislation.gov.au/C2004A01224/2019-02-24/2019-02-24/text/1/epub/OEBPS/document_1/document_1.html#_Toc1469220"^^xsd:anyURI ;
    dcat:theme legcons:Item .

C2004A01224:101 a legcons:Item,
        C2004A01224:Item,
        owl:Class,
        dcat:Resource ;
    rdfs:label "Item - I101 54  Instruments to which this Part does not apply"@en-AU ;
    dct:isPartOf C2004A01224:60 ;
    rdfs:comment "54  Instruments to which this Part does not apply - Abrievated Graph Key: I101"@en-AU ;
    rdfs:subClassOf C2004A01224: ;
    skos:definition "54  Instruments to which this Part does not apply"@en-AU ;
    skos:narrower C2004A01224:60 ;
    skos:prefLabel "Item I101"@en-AU ;
    dcat:accessURL <https://www.legislation.gov.au/C2004A01224/2019-02-24/2019-02-24/text/1/epub/OEBPS/document_1/document_1.html#_Toc1469221> ;
    dcat:landingPage "https://www.legislation.gov.au/C2004A01224/2019-02-24/2019-02-24/text/1/epub/OEBPS/document_1/document_1.html#_Toc1469221"^^xsd:anyURI ;
    dcat:theme legcons:Item .

C2004A01224:103 a legcons:Item,
        C2004A01224:Item,
        owl:Class,
        dcat:Resource ;
    rdfs:label "Item - I103 55  Simplified outline of this Chapter"@en-AU ;
    dct:isPartOf C2004A01224:102 ;
    rdfs:comment "55  Simplified outline of this Chapter - Abrievated Graph Key: I103"@en-AU ;
    rdfs:subClassOf C2004A01224: ;
    skos:definition "55  Simplified outline of this Chapter"@en-AU ;
    skos:narrower C2004A01224:102 ;
    skos:prefLabel "Item I103"@en-AU ;
    dcat:accessURL <https://www.legislation.gov.au/C2004A01224/2019-02-24/2019-02-24/text/1/epub/OEBPS/document_1/document_1.html#_Toc1469223> ;
    dcat:landingPage "https://www.legislation.gov.au/C2004A01224/2019-02-24/2019-02-24/text/1/epub/OEBPS/document_1/document_1.html#_Toc1469223"^^xsd:anyURI ;
    dcat:theme legcons:Item .

C2004A01224:104 a legcons:Item,
        C2004A01224:Item,
        owl:Class,
        dcat:Resource ;
    rdfs:label "Item - I104 56  Legislative instrumentsgazettal and other publication and notification requirements"@en-AU ;
    dct:isPartOf C2004A01224:102 ;
    rdfs:comment "56  Legislative instrumentsgazettal and other publication and notification requirements - Abrievated Graph Key: I104"@en-AU ;
    rdfs:subClassOf C2004A01224: ;
    skos:definition "56  Legislative instrumentsgazettal and other publication and notification requirements"@en-AU ;
    skos:narrower C2004A01224:102 ;
    skos:prefLabel "Item I104"@en-AU ;
    dcat:accessURL <https://www.legislation.gov.au/C2004A01224/2019-02-24/2019-02-24/text/1/epub/OEBPS/document_1/document_1.html#_Toc1469224> ;
    dcat:landingPage "https://www.legislation.gov.au/C2004A01224/2019-02-24/2019-02-24/text/1/epub/OEBPS/document_1/document_1.html#_Toc1469224"^^xsd:anyURI ;
    dcat:theme legcons:Item .

C2004A01224:105 a legcons:Item,
        C2004A01224:Item,
        owl:Class,
        dcat:Resource ;
    rdfs:label "Item - I105 57  Effect on existing tabling and disallowance requirements"@en-AU ;
    dct:isPartOf C2004A01224:102 ;
    rdfs:comment "57  Effect on existing tabling and disallowance requirements - Abrievated Graph Key: I105"@en-AU ;
    rdfs:subClassOf C2004A01224: ;
    skos:definition "57  Effect on existing tabling and disallowance requirements"@en-AU ;
    skos:narrower C2004A01224:102 ;
    skos:prefLabel "Item I105"@en-AU ;
    dcat:accessURL <https://www.legislation.gov.au/C2004A01224/2019-02-24/2019-02-24/text/1/epub/OEBPS/document_1/document_1.html#_Toc1469225> ;
    dcat:landingPage "https://www.legislation.gov.au/C2004A01224/2019-02-24/2019-02-24/text/1/epub/OEBPS/document_1/document_1.html#_Toc1469225"^^xsd:anyURI ;
    dcat:theme legcons:Item .

C2004A01224:106 a legcons:Item,
        C2004A01224:Item,
        owl:Class,
        dcat:Resource ;
    rdfs:label "Item - I106 57 A  Legislative instruments made under power delegated by the Parliament before 1 January 2005"@en-AU ;
    dct:isPartOf C2004A01224:102 ;
    rdfs:comment "57 A  Legislative instruments made under power delegated by the Parliament before 1 January 2005 - Abrievated Graph Key: I106"@en-AU ;
    rdfs:subClassOf C2004A01224: ;
    skos:definition "57 A  Legislative instruments made under power delegated by the Parliament before 1 January 2005"@en-AU ;
    skos:narrower C2004A01224:102 ;
    skos:prefLabel "Item I106"@en-AU ;
    dcat:accessURL <https://www.legislation.gov.au/C2004A01224/2019-02-24/2019-02-24/text/1/epub/OEBPS/document_1/document_1.html#_Toc1469226> ;
    dcat:landingPage "https://www.legislation.gov.au/C2004A01224/2019-02-24/2019-02-24/text/1/epub/OEBPS/document_1/document_1.html#_Toc1469226"^^xsd:anyURI ;
    dcat:theme legcons:Item .

C2004A01224:107 a legcons:Item,
        C2004A01224:Item,
        owl:Class,
        dcat:Resource ;
    rdfs:label "Item - I107 58  Delegation"@en-AU ;
    dct:isPartOf C2004A01224:102 ;
    rdfs:comment "58  Delegation - Abrievated Graph Key: I107"@en-AU ;
    rdfs:subClassOf C2004A01224: ;
    skos:definition "58  Delegation"@en-AU ;
    skos:narrower C2004A01224:102 ;
    skos:prefLabel "Item I107"@en-AU ;
    dcat:accessURL <https://www.legislation.gov.au/C2004A01224/2019-02-24/2019-02-24/text/1/epub/OEBPS/document_1/document_1.html#_Toc1469227> ;
    dcat:landingPage "https://www.legislation.gov.au/C2004A01224/2019-02-24/2019-02-24/text/1/epub/OEBPS/document_1/document_1.html#_Toc1469227"^^xsd:anyURI ;
    dcat:theme legcons:Item .

C2004A01224:108 a legcons:Item,
        C2004A01224:Item,
        owl:Class,
        dcat:Resource ;
    rdfs:label "Item - I108 59  Review of operation of this Act"@en-AU ;
    dct:isPartOf C2004A01224:102 ;
    rdfs:comment "59  Review of operation of this Act - Abrievated Graph Key: I108"@en-AU ;
    rdfs:subClassOf C2004A01224: ;
    skos:definition "59  Review of operation of this Act"@en-AU ;
    skos:narrower C2004A01224:102 ;
    skos:prefLabel "Item I108"@en-AU ;
    dcat:accessURL <https://www.legislation.gov.au/C2004A01224/2019-02-24/2019-02-24/text/1/epub/OEBPS/document_1/document_1.html#_Toc1469228> ;
    dcat:landingPage "https://www.legislation.gov.au/C2004A01224/2019-02-24/2019-02-24/text/1/epub/OEBPS/document_1/document_1.html#_Toc1469228"^^xsd:anyURI ;
    dcat:theme legcons:Item .

C2004A01224:109 a legcons:Item,
        C2004A01224:Item,
        owl:Class,
        dcat:Resource ;
    rdfs:label "Item - I109 60  Review of operation of the sunsetting provisions"@en-AU ;
    dct:isPartOf C2004A01224:102 ;
    rdfs:comment "60  Review of operation of the sunsetting provisions - Abrievated Graph Key: I109"@en-AU ;
    rdfs:subClassOf C2004A01224: ;
    skos:definition "60  Review of operation of the sunsetting provisions"@en-AU ;
    skos:narrower C2004A01224:102 ;
    skos:prefLabel "Item I109"@en-AU ;
    dcat:accessURL <https://www.legislation.gov.au/C2004A01224/2019-02-24/2019-02-24/text/1/epub/OEBPS/document_1/document_1.html#_Toc1469229> ;
    dcat:landingPage "https://www.legislation.gov.au/C2004A01224/2019-02-24/2019-02-24/text/1/epub/OEBPS/document_1/document_1.html#_Toc1469229"^^xsd:anyURI ;
    dcat:theme legcons:Item .

C2004A01224:11 a legcons:Part,
        C2004A01224:Part,
        owl:Class,
        dcat:Resource ;
    rdfs:label "Part - P11 Part 2 Key concepts for legislative instruments and notifiable instruments"@en-AU ;
    dct:isPartOf C2004A01224:1 ;
    rdfs:comment "Part 2 Key concepts for legislative instruments and notifiable instruments - Abrievated Graph Key: P11"@en-AU ;
    rdfs:subClassOf C2004A01224: ;
    skos:definition "Part 2 Key concepts for legislative instruments and notifiable instruments"@en-AU ;
    skos:narrower C2004A01224:1 ;
    skos:prefLabel "Part P11"@en-AU ;
    dcat:accessURL <https://www.legislation.gov.au/C2004A01224/2019-02-24/2019-02-24/text/1/epub/OEBPS/document_1/document_1.html#_Toc1469131> ;
    dcat:landingPage "https://www.legislation.gov.au/C2004A01224/2019-02-24/2019-02-24/text/1/epub/OEBPS/document_1/document_1.html#_Toc1469131"^^xsd:anyURI ;
    dcat:theme legcons:Part .

C2004A01224:110 a legcons:Item,
        C2004A01224:Item,
        owl:Class,
        dcat:Resource ;
    rdfs:label "Item - I110 61  Legislative instrument and notifiable instrument amendments by regulations under this Act"@en-AU ;
    dct:isPartOf C2004A01224:102 ;
    rdfs:comment "61  Legislative instrument and notifiable instrument amendments by regulations under this Act - Abrievated Graph Key: I110"@en-AU ;
    rdfs:subClassOf C2004A01224: ;
    skos:definition "61  Legislative instrument and notifiable instrument amendments by regulations under this Act"@en-AU ;
    skos:narrower C2004A01224:102 ;
    skos:prefLabel "Item I110"@en-AU ;
    dcat:accessURL <https://www.legislation.gov.au/C2004A01224/2019-02-24/2019-02-24/text/1/epub/OEBPS/document_1/document_1.html#_Toc1469230> ;
    dcat:landingPage "https://www.legislation.gov.au/C2004A01224/2019-02-24/2019-02-24/text/1/epub/OEBPS/document_1/document_1.html#_Toc1469230"^^xsd:anyURI ;
    dcat:theme legcons:Item .

C2004A01224:111 a legcons:Item,
        C2004A01224:Item,
        owl:Class,
        dcat:Resource ;
    rdfs:label "Item - I111 61 A  Rules made by First Parliamentary Counsel"@en-AU ;
    dct:isPartOf C2004A01224:102 ;
    rdfs:comment "61 A  Rules made by First Parliamentary Counsel - Abrievated Graph Key: I111"@en-AU ;
    rdfs:subClassOf C2004A01224: ;
    skos:definition "61 A  Rules made by First Parliamentary Counsel"@en-AU ;
    skos:narrower C2004A01224:102 ;
    skos:prefLabel "Item I111"@en-AU ;
    dcat:accessURL <https://www.legislation.gov.au/C2004A01224/2019-02-24/2019-02-24/text/1/epub/OEBPS/document_1/document_1.html#_Toc1469231> ;
    dcat:landingPage "https://www.legislation.gov.au/C2004A01224/2019-02-24/2019-02-24/text/1/epub/OEBPS/document_1/document_1.html#_Toc1469231"^^xsd:anyURI ;
    dcat:theme legcons:Item .

C2004A01224:112 a legcons:Item,
        C2004A01224:Item,
        owl:Class,
        dcat:Resource ;
    rdfs:label "Item - I112 62  Regulations"@en-AU ;
    dct:isPartOf C2004A01224:102 ;
    rdfs:comment "62  Regulations - Abrievated Graph Key: I112"@en-AU ;
    rdfs:subClassOf C2004A01224: ;
    skos:definition "62  Regulations"@en-AU ;
    skos:narrower C2004A01224:102 ;
    skos:prefLabel "Item I112"@en-AU ;
    dcat:accessURL <https://www.legislation.gov.au/C2004A01224/2019-02-24/2019-02-24/text/1/epub/OEBPS/document_1/document_1.html#_Toc1469232> ;
    dcat:landingPage "https://www.legislation.gov.au/C2004A01224/2019-02-24/2019-02-24/text/1/epub/OEBPS/document_1/document_1.html#_Toc1469232"^^xsd:anyURI ;
    dcat:theme legcons:Item .

C2004A01224:114 a legcons:Item,
        C2004A01224:Item,
        owl:Class,
        dcat:Resource ;
    rdfs:label "Item - I114 Endnote 1 About the endnotes"@en-AU ;
    dct:isPartOf C2004A01224:113 ;
    rdfs:comment "Endnote 1 About the endnotes - Abrievated Graph Key: I114"@en-AU ;
    rdfs:subClassOf C2004A01224: ;
    skos:definition "Endnote 1 About the endnotes"@en-AU ;
    skos:narrower C2004A01224:113 ;
    skos:prefLabel "Item I114"@en-AU ;
    dcat:accessURL <https://www.legislation.gov.au/C2004A01224/2019-02-24/2019-02-24/text/1/epub/OEBPS/document_1/document_1.html#_Toc1469234> ;
    dcat:landingPage "https://www.legislation.gov.au/C2004A01224/2019-02-24/2019-02-24/text/1/epub/OEBPS/document_1/document_1.html#_Toc1469234"^^xsd:anyURI ;
    dcat:theme legcons:Item .

C2004A01224:115 a legcons:Item,
        C2004A01224:Item,
        owl:Class,
        dcat:Resource ;
    rdfs:label "Item - I115 Endnote 2 Abbreviation key"@en-AU ;
    dct:isPartOf C2004A01224:113 ;
    rdfs:comment "Endnote 2 Abbreviation key - Abrievated Graph Key: I115"@en-AU ;
    rdfs:subClassOf C2004A01224: ;
    skos:definition "Endnote 2 Abbreviation key"@en-AU ;
    skos:narrower C2004A01224:113 ;
    skos:prefLabel "Item I115"@en-AU ;
    dcat:accessURL <https://www.legislation.gov.au/C2004A01224/2019-02-24/2019-02-24/text/1/epub/OEBPS/document_1/document_1.html#_Toc1469235> ;
    dcat:landingPage "https://www.legislation.gov.au/C2004A01224/2019-02-24/2019-02-24/text/1/epub/OEBPS/document_1/document_1.html#_Toc1469235"^^xsd:anyURI ;
    dcat:theme legcons:Item .

C2004A01224:116 a legcons:Item,
        C2004A01224:Item,
        owl:Class,
        dcat:Resource ;
    rdfs:label "Item - I116 Endnote 3 Legislation history"@en-AU ;
    dct:isPartOf C2004A01224:113 ;
    rdfs:comment "Endnote 3 Legislation history - Abrievated Graph Key: I116"@en-AU ;
    rdfs:subClassOf C2004A01224: ;
    skos:definition "Endnote 3 Legislation history"@en-AU ;
    skos:narrower C2004A01224:113 ;
    skos:prefLabel "Item I116"@en-AU ;
    dcat:accessURL <https://www.legislation.gov.au/C2004A01224/2019-02-24/2019-02-24/text/1/epub/OEBPS/document_1/document_1.html#_Toc1469236> ;
    dcat:landingPage "https://www.legislation.gov.au/C2004A01224/2019-02-24/2019-02-24/text/1/epub/OEBPS/document_1/document_1.html#_Toc1469236"^^xsd:anyURI ;
    dcat:theme legcons:Item .

C2004A01224:117 a legcons:Item,
        C2004A01224:Item,
        owl:Class,
        dcat:Resource ;
    rdfs:label "Item - I117 Endnote 4 Amendment history"@en-AU ;
    dct:isPartOf C2004A01224:113 ;
    rdfs:comment "Endnote 4 Amendment history - Abrievated Graph Key: I117"@en-AU ;
    rdfs:subClassOf C2004A01224: ;
    skos:definition "Endnote 4 Amendment history"@en-AU ;
    skos:narrower C2004A01224:113 ;
    skos:prefLabel "Item I117"@en-AU ;
    dcat:accessURL <https://www.legislation.gov.au/C2004A01224/2019-02-24/2019-02-24/text/1/epub/OEBPS/document_1/document_1.html#_Toc1469237> ;
    dcat:landingPage "https://www.legislation.gov.au/C2004A01224/2019-02-24/2019-02-24/text/1/epub/OEBPS/document_1/document_1.html#_Toc1469237"^^xsd:anyURI ;
    dcat:theme legcons:Item .

C2004A01224:118 a legcons:Item,
        C2004A01224:Item,
        owl:Class,
        dcat:Resource ;
    rdfs:label "Item - I118 Endnote 5 Editorial changes"@en-AU ;
    dct:isPartOf C2004A01224:113 ;
    rdfs:comment "Endnote 5 Editorial changes - Abrievated Graph Key: I118"@en-AU ;
    rdfs:subClassOf C2004A01224: ;
    skos:definition "Endnote 5 Editorial changes"@en-AU ;
    skos:narrower C2004A01224:113 ;
    skos:prefLabel "Item I118"@en-AU ;
    dcat:accessURL <https://www.legislation.gov.au/C2004A01224/2019-02-24/2019-02-24/text/1/epub/OEBPS/document_1/document_1.html#_Toc1469238> ;
    dcat:landingPage "https://www.legislation.gov.au/C2004A01224/2019-02-24/2019-02-24/text/1/epub/OEBPS/document_1/document_1.html#_Toc1469238"^^xsd:anyURI ;
    dcat:theme legcons:Item .

C2004A01224:12 a legcons:Item,
        C2004A01224:Item,
        owl:Class,
        dcat:Resource ;
    rdfs:label "Item - I12 7  Simplified outline of this Part"@en-AU ;
    dct:isPartOf C2004A01224:1 ;
    rdfs:comment "7  Simplified outline of this Part - Abrievated Graph Key: I12"@en-AU ;
    rdfs:subClassOf C2004A01224: ;
    skos:definition "7  Simplified outline of this Part"@en-AU ;
    skos:narrower C2004A01224:1 ;
    skos:prefLabel "Item I12"@en-AU ;
    dcat:accessURL <https://www.legislation.gov.au/C2004A01224/2019-02-24/2019-02-24/text/1/epub/OEBPS/document_1/document_1.html#_Toc1469132> ;
    dcat:landingPage "https://www.legislation.gov.au/C2004A01224/2019-02-24/2019-02-24/text/1/epub/OEBPS/document_1/document_1.html#_Toc1469132"^^xsd:anyURI ;
    dcat:theme legcons:Item .

C2004A01224:13 a legcons:Item,
        C2004A01224:Item,
        owl:Class,
        dcat:Resource ;
    rdfs:label "Item - I13 8  Definition of legislative instrument"@en-AU ;
    dct:isPartOf C2004A01224:1 ;
    rdfs:comment "8  Definition of legislative instrument - Abrievated Graph Key: I13"@en-AU ;
    rdfs:subClassOf C2004A01224: ;
    skos:definition "8  Definition of legislative instrument"@en-AU ;
    skos:narrower C2004A01224:1 ;
    skos:prefLabel "Item I13"@en-AU ;
    dcat:accessURL <https://www.legislation.gov.au/C2004A01224/2019-02-24/2019-02-24/text/1/epub/OEBPS/document_1/document_1.html#_Toc1469133> ;
    dcat:landingPage "https://www.legislation.gov.au/C2004A01224/2019-02-24/2019-02-24/text/1/epub/OEBPS/document_1/document_1.html#_Toc1469133"^^xsd:anyURI ;
    dcat:theme legcons:Item .

C2004A01224:14 a legcons:Item,
        C2004A01224:Item,
        owl:Class,
        dcat:Resource ;
    rdfs:label "Item - I14 9  Inference of legislative character"@en-AU ;
    dct:isPartOf C2004A01224:1 ;
    rdfs:comment "9  Inference of legislative character - Abrievated Graph Key: I14"@en-AU ;
    rdfs:subClassOf C2004A01224: ;
    skos:definition "9  Inference of legislative character"@en-AU ;
    skos:narrower C2004A01224:1 ;
    skos:prefLabel "Item I14"@en-AU ;
    dcat:accessURL <https://www.legislation.gov.au/C2004A01224/2019-02-24/2019-02-24/text/1/epub/OEBPS/document_1/document_1.html#_Toc1469134> ;
    dcat:landingPage "https://www.legislation.gov.au/C2004A01224/2019-02-24/2019-02-24/text/1/epub/OEBPS/document_1/document_1.html#_Toc1469134"^^xsd:anyURI ;
    dcat:theme legcons:Item .

C2004A01224:15 a legcons:Item,
        C2004A01224:Item,
        owl:Class,
        dcat:Resource ;
    rdfs:label "Item - I15 10  Instruments declared to be legislative instruments"@en-AU ;
    dct:isPartOf C2004A01224:1 ;
    rdfs:comment "10  Instruments declared to be legislative instruments - Abrievated Graph Key: I15"@en-AU ;
    rdfs:subClassOf C2004A01224: ;
    skos:definition "10  Instruments declared to be legislative instruments"@en-AU ;
    skos:narrower C2004A01224:1 ;
    skos:prefLabel "Item I15"@en-AU ;
    dcat:accessURL <https://www.legislation.gov.au/C2004A01224/2019-02-24/2019-02-24/text/1/epub/OEBPS/document_1/document_1.html#_Toc1469135> ;
    dcat:landingPage "https://www.legislation.gov.au/C2004A01224/2019-02-24/2019-02-24/text/1/epub/OEBPS/document_1/document_1.html#_Toc1469135"^^xsd:anyURI ;
    dcat:theme legcons:Item .

C2004A01224:16 a legcons:Item,
        C2004A01224:Item,
        owl:Class,
        dcat:Resource ;
    rdfs:label "Item - I16 11  Definition of notifiable instrument"@en-AU ;
    dct:isPartOf C2004A01224:1 ;
    rdfs:comment "11  Definition of notifiable instrument - Abrievated Graph Key: I16"@en-AU ;
    rdfs:subClassOf C2004A01224: ;
    skos:definition "11  Definition of notifiable instrument"@en-AU ;
    skos:narrower C2004A01224:1 ;
    skos:prefLabel "Item I16"@en-AU ;
    dcat:accessURL <https://www.legislation.gov.au/C2004A01224/2019-02-24/2019-02-24/text/1/epub/OEBPS/document_1/document_1.html#_Toc1469136> ;
    dcat:landingPage "https://www.legislation.gov.au/C2004A01224/2019-02-24/2019-02-24/text/1/epub/OEBPS/document_1/document_1.html#_Toc1469136"^^xsd:anyURI ;
    dcat:theme legcons:Item .

C2004A01224:17 a legcons:Item,
        C2004A01224:Item,
        owl:Class,
        dcat:Resource ;
    rdfs:label "Item - I17 12  Commencement of legislative instruments and notifiable instruments"@en-AU ;
    dct:isPartOf C2004A01224:1 ;
    rdfs:comment "12  Commencement of legislative instruments and notifiable instruments - Abrievated Graph Key: I17"@en-AU ;
    rdfs:subClassOf C2004A01224: ;
    skos:definition "12  Commencement of legislative instruments and notifiable instruments"@en-AU ;
    skos:narrower C2004A01224:1 ;
    skos:prefLabel "Item I17"@en-AU ;
    dcat:accessURL <https://www.legislation.gov.au/C2004A01224/2019-02-24/2019-02-24/text/1/epub/OEBPS/document_1/document_1.html#_Toc1469137> ;
    dcat:landingPage "https://www.legislation.gov.au/C2004A01224/2019-02-24/2019-02-24/text/1/epub/OEBPS/document_1/document_1.html#_Toc1469137"^^xsd:anyURI ;
    dcat:theme legcons:Item .

C2004A01224:18 a legcons:Item,
        C2004A01224:Item,
        owl:Class,
        dcat:Resource ;
    rdfs:label "Item - I18 13  Construction of legislative instruments and notifiable instruments"@en-AU ;
    dct:isPartOf C2004A01224:1 ;
    rdfs:comment "13  Construction of legislative instruments and notifiable instruments - Abrievated Graph Key: I18"@en-AU ;
    rdfs:subClassOf C2004A01224: ;
    skos:definition "13  Construction of legislative instruments and notifiable instruments"@en-AU ;
    skos:narrower C2004A01224:1 ;
    skos:prefLabel "Item I18"@en-AU ;
    dcat:accessURL <https://www.legislation.gov.au/C2004A01224/2019-02-24/2019-02-24/text/1/epub/OEBPS/document_1/document_1.html#_Toc1469138> ;
    dcat:landingPage "https://www.legislation.gov.au/C2004A01224/2019-02-24/2019-02-24/text/1/epub/OEBPS/document_1/document_1.html#_Toc1469138"^^xsd:anyURI ;
    dcat:theme legcons:Item .

C2004A01224:19 a legcons:Item,
        C2004A01224:Item,
        owl:Class,
        dcat:Resource ;
    rdfs:label "Item - I19 14  Prescribing matters by reference to other instruments"@en-AU ;
    dct:isPartOf C2004A01224:1 ;
    rdfs:comment "14  Prescribing matters by reference to other instruments - Abrievated Graph Key: I19"@en-AU ;
    rdfs:subClassOf C2004A01224: ;
    skos:definition "14  Prescribing matters by reference to other instruments"@en-AU ;
    skos:narrower C2004A01224:1 ;
    skos:prefLabel "Item I19"@en-AU ;
    dcat:accessURL <https://www.legislation.gov.au/C2004A01224/2019-02-24/2019-02-24/text/1/epub/OEBPS/document_1/document_1.html#_Toc1469139> ;
    dcat:landingPage "https://www.legislation.gov.au/C2004A01224/2019-02-24/2019-02-24/text/1/epub/OEBPS/document_1/document_1.html#_Toc1469139"^^xsd:anyURI ;
    dcat:theme legcons:Item .

C2004A01224:2 a legcons:Part,
        C2004A01224:Part,
        owl:Class,
        dcat:Resource ;
    rdfs:label "Part - P2 Part 1 Preliminary"@en-AU ;
    dct:isPartOf C2004A01224:1 ;
    rdfs:comment "Part 1 Preliminary - Abrievated Graph Key: P2"@en-AU ;
    rdfs:subClassOf C2004A01224: ;
    skos:definition "Part 1 Preliminary"@en-AU ;
    skos:narrower C2004A01224:1 ;
    skos:prefLabel "Part P2"@en-AU ;
    dcat:accessURL <https://www.legislation.gov.au/C2004A01224/2019-02-24/2019-02-24/text/1/epub/OEBPS/document_1/document_1.html#_Toc1469122> ;
    dcat:landingPage "https://www.legislation.gov.au/C2004A01224/2019-02-24/2019-02-24/text/1/epub/OEBPS/document_1/document_1.html#_Toc1469122"^^xsd:anyURI ;
    dcat:theme legcons:Part .

C2004A01224:23 a legcons:Item,
        C2004A01224:Item,
        owl:Class,
        dcat:Resource ;
    rdfs:label "Item - I23 15  Simplified outline of this Part"@en-AU ;
    dct:isPartOf C2004A01224:22 ;
    rdfs:comment "15  Simplified outline of this Part - Abrievated Graph Key: I23"@en-AU ;
    rdfs:subClassOf C2004A01224: ;
    skos:definition "15  Simplified outline of this Part"@en-AU ;
    skos:narrower C2004A01224:22 ;
    skos:prefLabel "Item I23"@en-AU ;
    dcat:accessURL <https://www.legislation.gov.au/C2004A01224/2019-02-24/2019-02-24/text/1/epub/OEBPS/document_1/document_1.html#_Toc1469143> ;
    dcat:landingPage "https://www.legislation.gov.au/C2004A01224/2019-02-24/2019-02-24/text/1/epub/OEBPS/document_1/document_1.html#_Toc1469143"^^xsd:anyURI ;
    dcat:theme legcons:Item .

C2004A01224:24 a legcons:Division,
        C2004A01224:Division,
        owl:Class,
        dcat:Resource ;
    rdfs:label "Division - D24 Division 2 Federal Register of Legislation"@en-AU ;
    dct:isPartOf C2004A01224:21 ;
    rdfs:comment "Division 2 Federal Register of Legislation - Abrievated Graph Key: D24"@en-AU ;
    rdfs:subClassOf C2004A01224: ;
    skos:definition "Division 2 Federal Register of Legislation"@en-AU ;
    skos:narrower C2004A01224:21 ;
    skos:prefLabel "Division D24"@en-AU ;
    dcat:accessURL <https://www.legislation.gov.au/C2004A01224/2019-02-24/2019-02-24/text/1/epub/OEBPS/document_1/document_1.html#_Toc1469144> ;
    dcat:landingPage "https://www.legislation.gov.au/C2004A01224/2019-02-24/2019-02-24/text/1/epub/OEBPS/document_1/document_1.html#_Toc1469144"^^xsd:anyURI ;
    dcat:theme legcons:Division .

C2004A01224:25 a legcons:Item,
        C2004A01224:Item,
        owl:Class,
        dcat:Resource ;
    rdfs:label "Item - I25 15 A  Federal Register of Legislationestablishment and maintenance"@en-AU ;
    dct:isPartOf C2004A01224:21 ;
    rdfs:comment "15 A  Federal Register of Legislationestablishment and maintenance - Abrievated Graph Key: I25"@en-AU ;
    rdfs:subClassOf C2004A01224: ;
    skos:definition "15 A  Federal Register of Legislationestablishment and maintenance"@en-AU ;
    skos:narrower C2004A01224:21 ;
    skos:prefLabel "Item I25"@en-AU ;
    dcat:accessURL <https://www.legislation.gov.au/C2004A01224/2019-02-24/2019-02-24/text/1/epub/OEBPS/document_1/document_1.html#_Toc1469145> ;
    dcat:landingPage "https://www.legislation.gov.au/C2004A01224/2019-02-24/2019-02-24/text/1/epub/OEBPS/document_1/document_1.html#_Toc1469145"^^xsd:anyURI ;
    dcat:theme legcons:Item .

C2004A01224:26 a legcons:Item,
        C2004A01224:Item,
        owl:Class,
        dcat:Resource ;
    rdfs:label "Item - I26 15 B  Federal Register of Legislationcomplete record of registered laws"@en-AU ;
    dct:isPartOf C2004A01224:21 ;
    rdfs:comment "15 B  Federal Register of Legislationcomplete record of registered laws - Abrievated Graph Key: I26"@en-AU ;
    rdfs:subClassOf C2004A01224: ;
    skos:definition "15 B  Federal Register of Legislationcomplete record of registered laws"@en-AU ;
    skos:narrower C2004A01224:21 ;
    skos:prefLabel "Item I26"@en-AU ;
    dcat:accessURL <https://www.legislation.gov.au/C2004A01224/2019-02-24/2019-02-24/text/1/epub/OEBPS/document_1/document_1.html#_Toc1469146> ;
    dcat:landingPage "https://www.legislation.gov.au/C2004A01224/2019-02-24/2019-02-24/text/1/epub/OEBPS/document_1/document_1.html#_Toc1469146"^^xsd:anyURI ;
    dcat:theme legcons:Item .

C2004A01224:27 a legcons:Item,
        C2004A01224:Item,
        owl:Class,
        dcat:Resource ;
    rdfs:label "Item - I27 15 C  Federal Register of Legislationaccess to registered material on approved website"@en-AU ;
    dct:isPartOf C2004A01224:21 ;
    rdfs:comment "15 C  Federal Register of Legislationaccess to registered material on approved website - Abrievated Graph Key: I27"@en-AU ;
    rdfs:subClassOf C2004A01224: ;
    skos:definition "15 C  Federal Register of Legislationaccess to registered material on approved website"@en-AU ;
    skos:narrower C2004A01224:21 ;
    skos:prefLabel "Item I27"@en-AU ;
    dcat:accessURL <https://www.legislation.gov.au/C2004A01224/2019-02-24/2019-02-24/text/1/epub/OEBPS/document_1/document_1.html#_Toc1469147> ;
    dcat:landingPage "https://www.legislation.gov.au/C2004A01224/2019-02-24/2019-02-24/text/1/epub/OEBPS/document_1/document_1.html#_Toc1469147"^^xsd:anyURI ;
    dcat:theme legcons:Item .

C2004A01224:28 a legcons:Item,
        C2004A01224:Item,
        owl:Class,
        dcat:Resource ;
    rdfs:label "Item - I28 15 D  Federal Register of Legislationrectification of Register"@en-AU ;
    dct:isPartOf C2004A01224:21 ;
    rdfs:comment "15 D  Federal Register of Legislationrectification of Register - Abrievated Graph Key: I28"@en-AU ;
    rdfs:subClassOf C2004A01224: ;
    skos:definition "15 D  Federal Register of Legislationrectification of Register"@en-AU ;
    skos:narrower C2004A01224:21 ;
    skos:prefLabel "Item I28"@en-AU ;
    dcat:accessURL <https://www.legislation.gov.au/C2004A01224/2019-02-24/2019-02-24/text/1/epub/OEBPS/document_1/document_1.html#_Toc1469148> ;
    dcat:landingPage "https://www.legislation.gov.au/C2004A01224/2019-02-24/2019-02-24/text/1/epub/OEBPS/document_1/document_1.html#_Toc1469148"^^xsd:anyURI ;
    dcat:theme legcons:Item .

C2004A01224:29 a legcons:Item,
        C2004A01224:Item,
        owl:Class,
        dcat:Resource ;
    rdfs:label "Item - I29 15 DA  Requirement for re tabling and new disallowance period after rectification of Register"@en-AU ;
    dct:isPartOf C2004A01224:21 ;
    rdfs:comment "15 DA  Requirement for re tabling and new disallowance period after rectification of Register - Abrievated Graph Key: I29"@en-AU ;
    rdfs:subClassOf C2004A01224: ;
    skos:definition "15 DA  Requirement for re tabling and new disallowance period after rectification of Register"@en-AU ;
    skos:narrower C2004A01224:21 ;
    skos:prefLabel "Item I29"@en-AU ;
    dcat:accessURL <https://www.legislation.gov.au/C2004A01224/2019-02-24/2019-02-24/text/1/epub/OEBPS/document_1/document_1.html#_Toc1469149> ;
    dcat:landingPage "https://www.legislation.gov.au/C2004A01224/2019-02-24/2019-02-24/text/1/epub/OEBPS/document_1/document_1.html#_Toc1469149"^^xsd:anyURI ;
    dcat:theme legcons:Item .

C2004A01224:3 a legcons:Item,
        C2004A01224:Item,
        owl:Class,
        dcat:Resource ;
    rdfs:label "Item - I3 1  Short title"@en-AU ;
    dct:isPartOf C2004A01224:1 ;
    rdfs:comment "1  Short title - Abrievated Graph Key: I3"@en-AU ;
    rdfs:subClassOf C2004A01224: ;
    skos:definition "1  Short title"@en-AU ;
    skos:narrower C2004A01224:1 ;
    skos:prefLabel "Item I3"@en-AU ;
    dcat:accessURL <https://www.legislation.gov.au/C2004A01224/2019-02-24/2019-02-24/text/1/epub/OEBPS/document_1/document_1.html#_Toc1469123> ;
    dcat:landingPage "https://www.legislation.gov.au/C2004A01224/2019-02-24/2019-02-24/text/1/epub/OEBPS/document_1/document_1.html#_Toc1469123"^^xsd:anyURI ;
    dcat:theme legcons:Item .

C2004A01224:30 a legcons:Item,
        C2004A01224:Item,
        owl:Class,
        dcat:Resource ;
    rdfs:label "Item - I30 15 E  Federal Register of Legislationkeeping the Register"@en-AU ;
    dct:isPartOf C2004A01224:21 ;
    rdfs:comment "15 E  Federal Register of Legislationkeeping the Register - Abrievated Graph Key: I30"@en-AU ;
    rdfs:subClassOf C2004A01224: ;
    skos:definition "15 E  Federal Register of Legislationkeeping the Register"@en-AU ;
    skos:narrower C2004A01224:21 ;
    skos:prefLabel "Item I30"@en-AU ;
    dcat:accessURL <https://www.legislation.gov.au/C2004A01224/2019-02-24/2019-02-24/text/1/epub/OEBPS/document_1/document_1.html#_Toc1469150> ;
    dcat:landingPage "https://www.legislation.gov.au/C2004A01224/2019-02-24/2019-02-24/text/1/epub/OEBPS/document_1/document_1.html#_Toc1469150"^^xsd:anyURI ;
    dcat:theme legcons:Item .

C2004A01224:31 a legcons:Division,
        C2004A01224:Division,
        owl:Class,
        dcat:Resource ;
    rdfs:label "Division - D31 Division 3 Registration on Federal Register of Legislation"@en-AU ;
    dct:isPartOf C2004A01224:21 ;
    rdfs:comment "Division 3 Registration on Federal Register of Legislation - Abrievated Graph Key: D31"@en-AU ;
    rdfs:subClassOf C2004A01224: ;
    skos:definition "Division 3 Registration on Federal Register of Legislation"@en-AU ;
    skos:narrower C2004A01224:21 ;
    skos:prefLabel "Division D31"@en-AU ;
    dcat:accessURL <https://www.legislation.gov.au/C2004A01224/2019-02-24/2019-02-24/text/1/epub/OEBPS/document_1/document_1.html#_Toc1469151> ;
    dcat:landingPage "https://www.legislation.gov.au/C2004A01224/2019-02-24/2019-02-24/text/1/epub/OEBPS/document_1/document_1.html#_Toc1469151"^^xsd:anyURI ;
    dcat:theme legcons:Division .

C2004A01224:32 a legcons:Item,
        C2004A01224:Item,
        owl:Class,
        dcat:Resource ;
    rdfs:label "Item - I32 15 F  Registration of Acts"@en-AU ;
    dct:isPartOf C2004A01224:21 ;
    rdfs:comment "15 F  Registration of Acts - Abrievated Graph Key: I32"@en-AU ;
    rdfs:subClassOf C2004A01224: ;
    skos:definition "15 F  Registration of Acts"@en-AU ;
    skos:narrower C2004A01224:21 ;
    skos:prefLabel "Item I32"@en-AU ;
    dcat:accessURL <https://www.legislation.gov.au/C2004A01224/2019-02-24/2019-02-24/text/1/epub/OEBPS/document_1/document_1.html#_Toc1469152> ;
    dcat:landingPage "https://www.legislation.gov.au/C2004A01224/2019-02-24/2019-02-24/text/1/epub/OEBPS/document_1/document_1.html#_Toc1469152"^^xsd:anyURI ;
    dcat:theme legcons:Item .

C2004A01224:33 a legcons:Item,
        C2004A01224:Item,
        owl:Class,
        dcat:Resource ;
    rdfs:label "Item - I33 15 G  Lodgement of legislative instruments and notifiable instruments and other material"@en-AU ;
    dct:isPartOf C2004A01224:21 ;
    rdfs:comment "15 G  Lodgement of legislative instruments and notifiable instruments and other material - Abrievated Graph Key: I33"@en-AU ;
    rdfs:subClassOf C2004A01224: ;
    skos:definition "15 G  Lodgement of legislative instruments and notifiable instruments and other material"@en-AU ;
    skos:narrower C2004A01224:21 ;
    skos:prefLabel "Item I33"@en-AU ;
    dcat:accessURL <https://www.legislation.gov.au/C2004A01224/2019-02-24/2019-02-24/text/1/epub/OEBPS/document_1/document_1.html#_Toc1469153> ;
    dcat:landingPage "https://www.legislation.gov.au/C2004A01224/2019-02-24/2019-02-24/text/1/epub/OEBPS/document_1/document_1.html#_Toc1469153"^^xsd:anyURI ;
    dcat:theme legcons:Item .

C2004A01224:34 a legcons:Item,
        C2004A01224:Item,
        owl:Class,
        dcat:Resource ;
    rdfs:label "Item - I34 15 H  Registration of legislative instruments and notifiable instruments and other documents"@en-AU ;
    dct:isPartOf C2004A01224:21 ;
    rdfs:comment "15 H  Registration of legislative instruments and notifiable instruments and other documents - Abrievated Graph Key: I34"@en-AU ;
    rdfs:subClassOf C2004A01224: ;
    skos:definition "15 H  Registration of legislative instruments and notifiable instruments and other documents"@en-AU ;
    skos:narrower C2004A01224:21 ;
    skos:prefLabel "Item I34"@en-AU ;
    dcat:accessURL <https://www.legislation.gov.au/C2004A01224/2019-02-24/2019-02-24/text/1/epub/OEBPS/document_1/document_1.html#_Toc1469154> ;
    dcat:landingPage "https://www.legislation.gov.au/C2004A01224/2019-02-24/2019-02-24/text/1/epub/OEBPS/document_1/document_1.html#_Toc1469154"^^xsd:anyURI ;
    dcat:theme legcons:Item .

C2004A01224:35 a legcons:Item,
        C2004A01224:Item,
        owl:Class,
        dcat:Resource ;
    rdfs:label "Item - I35 15 J  Explanatory statements"@en-AU ;
    dct:isPartOf C2004A01224:21 ;
    rdfs:comment "15 J  Explanatory statements - Abrievated Graph Key: I35"@en-AU ;
    rdfs:subClassOf C2004A01224: ;
    skos:definition "15 J  Explanatory statements"@en-AU ;
    skos:narrower C2004A01224:21 ;
    skos:prefLabel "Item I35"@en-AU ;
    dcat:accessURL <https://www.legislation.gov.au/C2004A01224/2019-02-24/2019-02-24/text/1/epub/OEBPS/document_1/document_1.html#_Toc1469155> ;
    dcat:landingPage "https://www.legislation.gov.au/C2004A01224/2019-02-24/2019-02-24/text/1/epub/OEBPS/document_1/document_1.html#_Toc1469155"^^xsd:anyURI ;
    dcat:theme legcons:Item .

C2004A01224:36 a legcons:Item,
        C2004A01224:Item,
        owl:Class,
        dcat:Resource ;
    rdfs:label "Item - I36 15 K  Registrationenforceability of legislative instruments"@en-AU ;
    dct:isPartOf C2004A01224:21 ;
    rdfs:comment "15 K  Registrationenforceability of legislative instruments - Abrievated Graph Key: I36"@en-AU ;
    rdfs:subClassOf C2004A01224: ;
    skos:definition "15 K  Registrationenforceability of legislative instruments"@en-AU ;
    skos:narrower C2004A01224:21 ;
    skos:prefLabel "Item I36"@en-AU ;
    dcat:accessURL <https://www.legislation.gov.au/C2004A01224/2019-02-24/2019-02-24/text/1/epub/OEBPS/document_1/document_1.html#_Toc1469156> ;
    dcat:landingPage "https://www.legislation.gov.au/C2004A01224/2019-02-24/2019-02-24/text/1/epub/OEBPS/document_1/document_1.html#_Toc1469156"^^xsd:anyURI ;
    dcat:theme legcons:Item .

C2004A01224:37 a legcons:Item,
        C2004A01224:Item,
        owl:Class,
        dcat:Resource ;
    rdfs:label "Item - I37 15 L  Events affecting the currency or accuracy of the Register"@en-AU ;
    dct:isPartOf C2004A01224:21 ;
    rdfs:comment "15 L  Events affecting the currency or accuracy of the Register - Abrievated Graph Key: I37"@en-AU ;
    rdfs:subClassOf C2004A01224: ;
    skos:definition "15 L  Events affecting the currency or accuracy of the Register"@en-AU ;
    skos:narrower C2004A01224:21 ;
    skos:prefLabel "Item I37"@en-AU ;
    dcat:accessURL <https://www.legislation.gov.au/C2004A01224/2019-02-24/2019-02-24/text/1/epub/OEBPS/document_1/document_1.html#_Toc1469157> ;
    dcat:landingPage "https://www.legislation.gov.au/C2004A01224/2019-02-24/2019-02-24/text/1/epub/OEBPS/document_1/document_1.html#_Toc1469157"^^xsd:anyURI ;
    dcat:theme legcons:Item .

C2004A01224:38 a legcons:Item,
        C2004A01224:Item,
        owl:Class,
        dcat:Resource ;
    rdfs:label "Item - I38 15 M  Rules for lodgement and registration"@en-AU ;
    dct:isPartOf C2004A01224:21 ;
    rdfs:comment "15 M  Rules for lodgement and registration - Abrievated Graph Key: I38"@en-AU ;
    rdfs:subClassOf C2004A01224: ;
    skos:definition "15 M  Rules for lodgement and registration"@en-AU ;
    skos:narrower C2004A01224:21 ;
    skos:prefLabel "Item I38"@en-AU ;
    dcat:accessURL <https://www.legislation.gov.au/C2004A01224/2019-02-24/2019-02-24/text/1/epub/OEBPS/document_1/document_1.html#_Toc1469158> ;
    dcat:landingPage "https://www.legislation.gov.au/C2004A01224/2019-02-24/2019-02-24/text/1/epub/OEBPS/document_1/document_1.html#_Toc1469158"^^xsd:anyURI ;
    dcat:theme legcons:Item .

C2004A01224:39 a legcons:Part,
        C2004A01224:Part,
        owl:Class,
        dcat:Resource ;
    rdfs:label "Part - P39 Part 2 Compilations"@en-AU ;
    dct:isPartOf C2004A01224:20 ;
    rdfs:comment "Part 2 Compilations - Abrievated Graph Key: P39"@en-AU ;
    rdfs:subClassOf C2004A01224: ;
    skos:definition "Part 2 Compilations"@en-AU ;
    skos:narrower C2004A01224:20 ;
    skos:prefLabel "Part P39"@en-AU ;
    dcat:accessURL <https://www.legislation.gov.au/C2004A01224/2019-02-24/2019-02-24/text/1/epub/OEBPS/document_1/document_1.html#_Toc1469159> ;
    dcat:landingPage "https://www.legislation.gov.au/C2004A01224/2019-02-24/2019-02-24/text/1/epub/OEBPS/document_1/document_1.html#_Toc1469159"^^xsd:anyURI ;
    dcat:theme legcons:Part .

C2004A01224:4 a legcons:Item,
        C2004A01224:Item,
        owl:Class,
        dcat:Resource ;
    rdfs:label "Item - I4 2  Commencement"@en-AU ;
    dct:isPartOf C2004A01224:1 ;
    rdfs:comment "2  Commencement - Abrievated Graph Key: I4"@en-AU ;
    rdfs:subClassOf C2004A01224: ;
    skos:definition "2  Commencement"@en-AU ;
    skos:narrower C2004A01224:1 ;
    skos:prefLabel "Item I4"@en-AU ;
    dcat:accessURL <https://www.legislation.gov.au/C2004A01224/2019-02-24/2019-02-24/text/1/epub/OEBPS/document_1/document_1.html#_Toc1469124> ;
    dcat:landingPage "https://www.legislation.gov.au/C2004A01224/2019-02-24/2019-02-24/text/1/epub/OEBPS/document_1/document_1.html#_Toc1469124"^^xsd:anyURI ;
    dcat:theme legcons:Item .

C2004A01224:41 a legcons:Item,
        C2004A01224:Item,
        owl:Class,
        dcat:Resource ;
    rdfs:label "Item - I41 15 N  Simplified outline of this Part"@en-AU ;
    dct:isPartOf C2004A01224:40 ;
    rdfs:comment "15 N  Simplified outline of this Part - Abrievated Graph Key: I41"@en-AU ;
    rdfs:subClassOf C2004A01224: ;
    skos:definition "15 N  Simplified outline of this Part"@en-AU ;
    skos:narrower C2004A01224:40 ;
    skos:prefLabel "Item I41"@en-AU ;
    dcat:accessURL <https://www.legislation.gov.au/C2004A01224/2019-02-24/2019-02-24/text/1/epub/OEBPS/document_1/document_1.html#_Toc1469161> ;
    dcat:landingPage "https://www.legislation.gov.au/C2004A01224/2019-02-24/2019-02-24/text/1/epub/OEBPS/document_1/document_1.html#_Toc1469161"^^xsd:anyURI ;
    dcat:theme legcons:Item .

C2004A01224:43 a legcons:Item,
        C2004A01224:Item,
        owl:Class,
        dcat:Resource ;
    rdfs:label "Item - I43 15 P  Registered compilationsinformation requirements"@en-AU ;
    dct:isPartOf C2004A01224:42 ;
    rdfs:comment "15 P  Registered compilationsinformation requirements - Abrievated Graph Key: I43"@en-AU ;
    rdfs:subClassOf C2004A01224: ;
    skos:definition "15 P  Registered compilationsinformation requirements"@en-AU ;
    skos:narrower C2004A01224:42 ;
    skos:prefLabel "Item I43"@en-AU ;
    dcat:accessURL <https://www.legislation.gov.au/C2004A01224/2019-02-24/2019-02-24/text/1/epub/OEBPS/document_1/document_1.html#_Toc1469163> ;
    dcat:landingPage "https://www.legislation.gov.au/C2004A01224/2019-02-24/2019-02-24/text/1/epub/OEBPS/document_1/document_1.html#_Toc1469163"^^xsd:anyURI ;
    dcat:theme legcons:Item .

C2004A01224:44 a legcons:Item,
        C2004A01224:Item,
        owl:Class,
        dcat:Resource ;
    rdfs:label "Item - I44 15 Q  Definitions of required compilation event and discretionary compilation event etc"@en-AU ;
    dct:isPartOf C2004A01224:42 ;
    rdfs:comment "15 Q  Definitions of required compilation event and discretionary compilation event etc - Abrievated Graph Key: I44"@en-AU ;
    rdfs:subClassOf C2004A01224: ;
    skos:definition "15 Q  Definitions of required compilation event and discretionary compilation event etc"@en-AU ;
    skos:narrower C2004A01224:42 ;
    skos:prefLabel "Item I44"@en-AU ;
    dcat:accessURL <https://www.legislation.gov.au/C2004A01224/2019-02-24/2019-02-24/text/1/epub/OEBPS/document_1/document_1.html#_Toc1469164> ;
    dcat:landingPage "https://www.legislation.gov.au/C2004A01224/2019-02-24/2019-02-24/text/1/epub/OEBPS/document_1/document_1.html#_Toc1469164"^^xsd:anyURI ;
    dcat:theme legcons:Item .

C2004A01224:45 a legcons:Item,
        C2004A01224:Item,
        owl:Class,
        dcat:Resource ;
    rdfs:label "Item - I45 15 R  Lodgement of compilations of instrumentsrequired compilation events"@en-AU ;
    dct:isPartOf C2004A01224:42 ;
    rdfs:comment "15 R  Lodgement of compilations of instrumentsrequired compilation events - Abrievated Graph Key: I45"@en-AU ;
    rdfs:subClassOf C2004A01224: ;
    skos:definition "15 R  Lodgement of compilations of instrumentsrequired compilation events"@en-AU ;
    skos:narrower C2004A01224:42 ;
    skos:prefLabel "Item I45"@en-AU ;
    dcat:accessURL <https://www.legislation.gov.au/C2004A01224/2019-02-24/2019-02-24/text/1/epub/OEBPS/document_1/document_1.html#_Toc1469165> ;
    dcat:landingPage "https://www.legislation.gov.au/C2004A01224/2019-02-24/2019-02-24/text/1/epub/OEBPS/document_1/document_1.html#_Toc1469165"^^xsd:anyURI ;
    dcat:theme legcons:Item .

C2004A01224:46 a legcons:Item,
        C2004A01224:Item,
        owl:Class,
        dcat:Resource ;
    rdfs:label "Item - I46 15 S  Lodgement of compilations of instrumentsdiscretionary compilation events"@en-AU ;
    dct:isPartOf C2004A01224:42 ;
    rdfs:comment "15 S  Lodgement of compilations of instrumentsdiscretionary compilation events - Abrievated Graph Key: I46"@en-AU ;
    rdfs:subClassOf C2004A01224: ;
    skos:definition "15 S  Lodgement of compilations of instrumentsdiscretionary compilation events"@en-AU ;
    skos:narrower C2004A01224:42 ;
    skos:prefLabel "Item I46"@en-AU ;
    dcat:accessURL <https://www.legislation.gov.au/C2004A01224/2019-02-24/2019-02-24/text/1/epub/OEBPS/document_1/document_1.html#_Toc1469166> ;
    dcat:landingPage "https://www.legislation.gov.au/C2004A01224/2019-02-24/2019-02-24/text/1/epub/OEBPS/document_1/document_1.html#_Toc1469166"^^xsd:anyURI ;
    dcat:theme legcons:Item .

C2004A01224:47 a legcons:Item,
        C2004A01224:Item,
        owl:Class,
        dcat:Resource ;
    rdfs:label "Item - I47 15 T  Registration of compilations"@en-AU ;
    dct:isPartOf C2004A01224:42 ;
    rdfs:comment "15 T  Registration of compilations - Abrievated Graph Key: I47"@en-AU ;
    rdfs:subClassOf C2004A01224: ;
    skos:definition "15 T  Registration of compilations"@en-AU ;
    skos:narrower C2004A01224:42 ;
    skos:prefLabel "Item I47"@en-AU ;
    dcat:accessURL <https://www.legislation.gov.au/C2004A01224/2019-02-24/2019-02-24/text/1/epub/OEBPS/document_1/document_1.html#_Toc1469167> ;
    dcat:landingPage "https://www.legislation.gov.au/C2004A01224/2019-02-24/2019-02-24/text/1/epub/OEBPS/document_1/document_1.html#_Toc1469167"^^xsd:anyURI ;
    dcat:theme legcons:Item .

C2004A01224:48 a legcons:Item,
        C2004A01224:Item,
        owl:Class,
        dcat:Resource ;
    rdfs:label "Item - I48 15 U  Compilationsrules"@en-AU ;
    dct:isPartOf C2004A01224:42 ;
    rdfs:comment "15 U  Compilationsrules - Abrievated Graph Key: I48"@en-AU ;
    rdfs:subClassOf C2004A01224: ;
    skos:definition "15 U  Compilationsrules"@en-AU ;
    skos:narrower C2004A01224:42 ;
    skos:prefLabel "Item I48"@en-AU ;
    dcat:accessURL <https://www.legislation.gov.au/C2004A01224/2019-02-24/2019-02-24/text/1/epub/OEBPS/document_1/document_1.html#_Toc1469168> ;
    dcat:landingPage "https://www.legislation.gov.au/C2004A01224/2019-02-24/2019-02-24/text/1/epub/OEBPS/document_1/document_1.html#_Toc1469168"^^xsd:anyURI ;
    dcat:theme legcons:Item .

C2004A01224:5 a legcons:Item,
        C2004A01224:Item,
        owl:Class,
        dcat:Resource ;
    rdfs:label "Item - I5 3  Object"@en-AU ;
    dct:isPartOf C2004A01224:1 ;
    rdfs:comment "3  Object - Abrievated Graph Key: I5"@en-AU ;
    rdfs:subClassOf C2004A01224: ;
    skos:definition "3  Object"@en-AU ;
    skos:narrower C2004A01224:1 ;
    skos:prefLabel "Item I5"@en-AU ;
    dcat:accessURL <https://www.legislation.gov.au/C2004A01224/2019-02-24/2019-02-24/text/1/epub/OEBPS/document_1/document_1.html#_Toc1469125> ;
    dcat:landingPage "https://www.legislation.gov.au/C2004A01224/2019-02-24/2019-02-24/text/1/epub/OEBPS/document_1/document_1.html#_Toc1469125"^^xsd:anyURI ;
    dcat:theme legcons:Item .

C2004A01224:50 a legcons:Item,
        C2004A01224:Item,
        owl:Class,
        dcat:Resource ;
    rdfs:label "Item - I50 15 V  Power to make editorial changes and other changes"@en-AU ;
    dct:isPartOf C2004A01224:49 ;
    rdfs:comment "15 V  Power to make editorial changes and other changes - Abrievated Graph Key: I50"@en-AU ;
    rdfs:subClassOf C2004A01224: ;
    skos:definition "15 V  Power to make editorial changes and other changes"@en-AU ;
    skos:narrower C2004A01224:49 ;
    skos:prefLabel "Item I50"@en-AU ;
    dcat:accessURL <https://www.legislation.gov.au/C2004A01224/2019-02-24/2019-02-24/text/1/epub/OEBPS/document_1/document_1.html#_Toc1469170> ;
    dcat:landingPage "https://www.legislation.gov.au/C2004A01224/2019-02-24/2019-02-24/text/1/epub/OEBPS/document_1/document_1.html#_Toc1469170"^^xsd:anyURI ;
    dcat:theme legcons:Item .

C2004A01224:51 a legcons:Item,
        C2004A01224:Item,
        owl:Class,
        dcat:Resource ;
    rdfs:label "Item - I51 15 W  Editorial changes treated in the same way as amendments"@en-AU ;
    dct:isPartOf C2004A01224:49 ;
    rdfs:comment "15 W  Editorial changes treated in the same way as amendments - Abrievated Graph Key: I51"@en-AU ;
    rdfs:subClassOf C2004A01224: ;
    skos:definition "15 W  Editorial changes treated in the same way as amendments"@en-AU ;
    skos:narrower C2004A01224:49 ;
    skos:prefLabel "Item I51"@en-AU ;
    dcat:accessURL <https://www.legislation.gov.au/C2004A01224/2019-02-24/2019-02-24/text/1/epub/OEBPS/document_1/document_1.html#_Toc1469171> ;
    dcat:landingPage "https://www.legislation.gov.au/C2004A01224/2019-02-24/2019-02-24/text/1/epub/OEBPS/document_1/document_1.html#_Toc1469171"^^xsd:anyURI ;
    dcat:theme legcons:Item .

C2004A01224:52 a legcons:Item,
        C2004A01224:Item,
        owl:Class,
        dcat:Resource ;
    rdfs:label "Item - I52 15 X  Definition of editorial change"@en-AU ;
    dct:isPartOf C2004A01224:49 ;
    rdfs:comment "15 X  Definition of editorial change - Abrievated Graph Key: I52"@en-AU ;
    rdfs:subClassOf C2004A01224: ;
    skos:definition "15 X  Definition of editorial change"@en-AU ;
    skos:narrower C2004A01224:49 ;
    skos:prefLabel "Item I52"@en-AU ;
    dcat:accessURL <https://www.legislation.gov.au/C2004A01224/2019-02-24/2019-02-24/text/1/epub/OEBPS/document_1/document_1.html#_Toc1469172> ;
    dcat:landingPage "https://www.legislation.gov.au/C2004A01224/2019-02-24/2019-02-24/text/1/epub/OEBPS/document_1/document_1.html#_Toc1469172"^^xsd:anyURI ;
    dcat:theme legcons:Item .

C2004A01224:53 a legcons:Part,
        C2004A01224:Part,
        owl:Class,
        dcat:Resource ;
    rdfs:label "Part - P53 Part 3 Authorised versions and judicial notice"@en-AU ;
    dct:isPartOf C2004A01224:20 ;
    rdfs:comment "Part 3 Authorised versions and judicial notice - Abrievated Graph Key: P53"@en-AU ;
    rdfs:subClassOf C2004A01224: ;
    skos:definition "Part 3 Authorised versions and judicial notice"@en-AU ;
    skos:narrower C2004A01224:20 ;
    skos:prefLabel "Part P53"@en-AU ;
    dcat:accessURL <https://www.legislation.gov.au/C2004A01224/2019-02-24/2019-02-24/text/1/epub/OEBPS/document_1/document_1.html#_Toc1469173> ;
    dcat:landingPage "https://www.legislation.gov.au/C2004A01224/2019-02-24/2019-02-24/text/1/epub/OEBPS/document_1/document_1.html#_Toc1469173"^^xsd:anyURI ;
    dcat:theme legcons:Part .

C2004A01224:55 a legcons:Item,
        C2004A01224:Item,
        owl:Class,
        dcat:Resource ;
    rdfs:label "Item - I55 15 Y  Simplified outline of this Part"@en-AU ;
    dct:isPartOf C2004A01224:54 ;
    rdfs:comment "15 Y  Simplified outline of this Part - Abrievated Graph Key: I55"@en-AU ;
    rdfs:subClassOf C2004A01224: ;
    skos:definition "15 Y  Simplified outline of this Part"@en-AU ;
    skos:narrower C2004A01224:54 ;
    skos:prefLabel "Item I55"@en-AU ;
    dcat:accessURL <https://www.legislation.gov.au/C2004A01224/2019-02-24/2019-02-24/text/1/epub/OEBPS/document_1/document_1.html#_Toc1469175> ;
    dcat:landingPage "https://www.legislation.gov.au/C2004A01224/2019-02-24/2019-02-24/text/1/epub/OEBPS/document_1/document_1.html#_Toc1469175"^^xsd:anyURI ;
    dcat:theme legcons:Item .

C2004A01224:56 a legcons:Item,
        C2004A01224:Item,
        owl:Class,
        dcat:Resource ;
    rdfs:label "Item - I56 15 Z  Scope of this Part"@en-AU ;
    dct:isPartOf C2004A01224:54 ;
    rdfs:comment "15 Z  Scope of this Part - Abrievated Graph Key: I56"@en-AU ;
    rdfs:subClassOf C2004A01224: ;
    skos:definition "15 Z  Scope of this Part"@en-AU ;
    skos:narrower C2004A01224:54 ;
    skos:prefLabel "Item I56"@en-AU ;
    dcat:accessURL <https://www.legislation.gov.au/C2004A01224/2019-02-24/2019-02-24/text/1/epub/OEBPS/document_1/document_1.html#_Toc1469176> ;
    dcat:landingPage "https://www.legislation.gov.au/C2004A01224/2019-02-24/2019-02-24/text/1/epub/OEBPS/document_1/document_1.html#_Toc1469176"^^xsd:anyURI ;
    dcat:theme legcons:Item .

C2004A01224:58 a legcons:Item,
        C2004A01224:Item,
        owl:Class,
        dcat:Resource ;
    rdfs:label "Item - I58 15 ZA  Authorised versions"@en-AU ;
    dct:isPartOf C2004A01224:57 ;
    rdfs:comment "15 ZA  Authorised versions - Abrievated Graph Key: I58"@en-AU ;
    rdfs:subClassOf C2004A01224: ;
    skos:definition "15 ZA  Authorised versions"@en-AU ;
    skos:narrower C2004A01224:57 ;
    skos:prefLabel "Item I58"@en-AU ;
    dcat:accessURL <https://www.legislation.gov.au/C2004A01224/2019-02-24/2019-02-24/text/1/epub/OEBPS/document_1/document_1.html#_Toc1469178> ;
    dcat:landingPage "https://www.legislation.gov.au/C2004A01224/2019-02-24/2019-02-24/text/1/epub/OEBPS/document_1/document_1.html#_Toc1469178"^^xsd:anyURI ;
    dcat:theme legcons:Item .

C2004A01224:59 a legcons:Item,
        C2004A01224:Item,
        owl:Class,
        dcat:Resource ;
    rdfs:label "Item - I59 15 ZB  Judicial notice"@en-AU ;
    dct:isPartOf C2004A01224:57 ;
    rdfs:comment "15 ZB  Judicial notice - Abrievated Graph Key: I59"@en-AU ;
    rdfs:subClassOf C2004A01224: ;
    skos:definition "15 ZB  Judicial notice"@en-AU ;
    skos:narrower C2004A01224:57 ;
    skos:prefLabel "Item I59"@en-AU ;
    dcat:accessURL <https://www.legislation.gov.au/C2004A01224/2019-02-24/2019-02-24/text/1/epub/OEBPS/document_1/document_1.html#_Toc1469179> ;
    dcat:landingPage "https://www.legislation.gov.au/C2004A01224/2019-02-24/2019-02-24/text/1/epub/OEBPS/document_1/document_1.html#_Toc1469179"^^xsd:anyURI ;
    dcat:theme legcons:Item .

C2004A01224:6 a legcons:Item,
        C2004A01224:Item,
        owl:Class,
        dcat:Resource ;
    rdfs:label "Item - I6 3 A  Simplified outline of this Act"@en-AU ;
    dct:isPartOf C2004A01224:1 ;
    rdfs:comment "3 A  Simplified outline of this Act - Abrievated Graph Key: I6"@en-AU ;
    rdfs:subClassOf C2004A01224: ;
    skos:definition "3 A  Simplified outline of this Act"@en-AU ;
    skos:narrower C2004A01224:1 ;
    skos:prefLabel "Item I6"@en-AU ;
    dcat:accessURL <https://www.legislation.gov.au/C2004A01224/2019-02-24/2019-02-24/text/1/epub/OEBPS/document_1/document_1.html#_Toc1469126> ;
    dcat:landingPage "https://www.legislation.gov.au/C2004A01224/2019-02-24/2019-02-24/text/1/epub/OEBPS/document_1/document_1.html#_Toc1469126"^^xsd:anyURI ;
    dcat:theme legcons:Item .

C2004A01224:62 a legcons:Item,
        C2004A01224:Item,
        owl:Class,
        dcat:Resource ;
    rdfs:label "Item - I62 15 ZC  Simplified outline of this Part"@en-AU ;
    dct:isPartOf C2004A01224:61 ;
    rdfs:comment "15 ZC  Simplified outline of this Part - Abrievated Graph Key: I62"@en-AU ;
    rdfs:subClassOf C2004A01224: ;
    skos:definition "15 ZC  Simplified outline of this Part"@en-AU ;
    skos:narrower C2004A01224:61 ;
    skos:prefLabel "Item I62"@en-AU ;
    dcat:accessURL <https://www.legislation.gov.au/C2004A01224/2019-02-24/2019-02-24/text/1/epub/OEBPS/document_1/document_1.html#_Toc1469182> ;
    dcat:landingPage "https://www.legislation.gov.au/C2004A01224/2019-02-24/2019-02-24/text/1/epub/OEBPS/document_1/document_1.html#_Toc1469182"^^xsd:anyURI ;
    dcat:theme legcons:Item .

C2004A01224:63 a legcons:Item,
        C2004A01224:Item,
        owl:Class,
        dcat:Resource ;
    rdfs:label "Item - I63 16  Measures to achieve high drafting standards for legislative instruments and notifiable instruments"@en-AU ;
    dct:isPartOf C2004A01224:61 ;
    rdfs:comment "16  Measures to achieve high drafting standards for legislative instruments and notifiable instruments - Abrievated Graph Key: I63"@en-AU ;
    rdfs:subClassOf C2004A01224: ;
    skos:definition "16  Measures to achieve high drafting standards for legislative instruments and notifiable instruments"@en-AU ;
    skos:narrower C2004A01224:61 ;
    skos:prefLabel "Item I63"@en-AU ;
    dcat:accessURL <https://www.legislation.gov.au/C2004A01224/2019-02-24/2019-02-24/text/1/epub/OEBPS/document_1/document_1.html#_Toc1469183> ;
    dcat:landingPage "https://www.legislation.gov.au/C2004A01224/2019-02-24/2019-02-24/text/1/epub/OEBPS/document_1/document_1.html#_Toc1469183"^^xsd:anyURI ;
    dcat:theme legcons:Item .

C2004A01224:64 a legcons:Item,
        C2004A01224:Item,
        owl:Class,
        dcat:Resource ;
    rdfs:label "Item - I64 17  Rule makers should consult before making legislative instruments"@en-AU ;
    dct:isPartOf C2004A01224:61 ;
    rdfs:comment "17  Rule makers should consult before making legislative instruments - Abrievated Graph Key: I64"@en-AU ;
    rdfs:subClassOf C2004A01224: ;
    skos:definition "17  Rule makers should consult before making legislative instruments"@en-AU ;
    skos:narrower C2004A01224:61 ;
    skos:prefLabel "Item I64"@en-AU ;
    dcat:accessURL <https://www.legislation.gov.au/C2004A01224/2019-02-24/2019-02-24/text/1/epub/OEBPS/document_1/document_1.html#_Toc1469184> ;
    dcat:landingPage "https://www.legislation.gov.au/C2004A01224/2019-02-24/2019-02-24/text/1/epub/OEBPS/document_1/document_1.html#_Toc1469184"^^xsd:anyURI ;
    dcat:theme legcons:Item .

C2004A01224:65 a legcons:Item,
        C2004A01224:Item,
        owl:Class,
        dcat:Resource ;
    rdfs:label "Item - I65 19  Consequence of failure to consult"@en-AU ;
    dct:isPartOf C2004A01224:61 ;
    rdfs:comment "19  Consequence of failure to consult - Abrievated Graph Key: I65"@en-AU ;
    rdfs:subClassOf C2004A01224: ;
    skos:definition "19  Consequence of failure to consult"@en-AU ;
    skos:narrower C2004A01224:61 ;
    skos:prefLabel "Item I65"@en-AU ;
    dcat:accessURL <https://www.legislation.gov.au/C2004A01224/2019-02-24/2019-02-24/text/1/epub/OEBPS/document_1/document_1.html#_Toc1469185> ;
    dcat:landingPage "https://www.legislation.gov.au/C2004A01224/2019-02-24/2019-02-24/text/1/epub/OEBPS/document_1/document_1.html#_Toc1469185"^^xsd:anyURI ;
    dcat:theme legcons:Item .

C2004A01224:67 a legcons:Item,
        C2004A01224:Item,
        owl:Class,
        dcat:Resource ;
    rdfs:label "Item - I67 36  Simplified outline of this Part"@en-AU ;
    dct:isPartOf C2004A01224:66 ;
    rdfs:comment "36  Simplified outline of this Part - Abrievated Graph Key: I67"@en-AU ;
    rdfs:subClassOf C2004A01224: ;
    skos:definition "36  Simplified outline of this Part"@en-AU ;
    skos:narrower C2004A01224:66 ;
    skos:prefLabel "Item I67"@en-AU ;
    dcat:accessURL <https://www.legislation.gov.au/C2004A01224/2019-02-24/2019-02-24/text/1/epub/OEBPS/document_1/document_1.html#_Toc1469187> ;
    dcat:landingPage "https://www.legislation.gov.au/C2004A01224/2019-02-24/2019-02-24/text/1/epub/OEBPS/document_1/document_1.html#_Toc1469187"^^xsd:anyURI ;
    dcat:theme legcons:Item .

C2004A01224:68 a legcons:Item,
        C2004A01224:Item,
        owl:Class,
        dcat:Resource ;
    rdfs:label "Item - I68 37  The purpose of the Part"@en-AU ;
    dct:isPartOf C2004A01224:66 ;
    rdfs:comment "37  The purpose of the Part - Abrievated Graph Key: I68"@en-AU ;
    rdfs:subClassOf C2004A01224: ;
    skos:definition "37  The purpose of the Part"@en-AU ;
    skos:narrower C2004A01224:66 ;
    skos:prefLabel "Item I68"@en-AU ;
    dcat:accessURL <https://www.legislation.gov.au/C2004A01224/2019-02-24/2019-02-24/text/1/epub/OEBPS/document_1/document_1.html#_Toc1469188> ;
    dcat:landingPage "https://www.legislation.gov.au/C2004A01224/2019-02-24/2019-02-24/text/1/epub/OEBPS/document_1/document_1.html#_Toc1469188"^^xsd:anyURI ;
    dcat:theme legcons:Item .

C2004A01224:69 a legcons:Item,
        C2004A01224:Item,
        owl:Class,
        dcat:Resource ;
    rdfs:label "Item - I69 38  Tabling of legislative instruments"@en-AU ;
    dct:isPartOf C2004A01224:66 ;
    rdfs:comment "38  Tabling of legislative instruments - Abrievated Graph Key: I69"@en-AU ;
    rdfs:subClassOf C2004A01224: ;
    skos:definition "38  Tabling of legislative instruments"@en-AU ;
    skos:narrower C2004A01224:66 ;
    skos:prefLabel "Item I69"@en-AU ;
    dcat:accessURL <https://www.legislation.gov.au/C2004A01224/2019-02-24/2019-02-24/text/1/epub/OEBPS/document_1/document_1.html#_Toc1469189> ;
    dcat:landingPage "https://www.legislation.gov.au/C2004A01224/2019-02-24/2019-02-24/text/1/epub/OEBPS/document_1/document_1.html#_Toc1469189"^^xsd:anyURI ;
    dcat:theme legcons:Item .

C2004A01224:7 a legcons:Item,
        C2004A01224:Item,
        owl:Class,
        dcat:Resource ;
    rdfs:label "Item - I7 3 AA  Norfolk Island"@en-AU ;
    dct:isPartOf C2004A01224:1 ;
    rdfs:comment "3 AA  Norfolk Island - Abrievated Graph Key: I7"@en-AU ;
    rdfs:subClassOf C2004A01224: ;
    skos:definition "3 AA  Norfolk Island"@en-AU ;
    skos:narrower C2004A01224:1 ;
    skos:prefLabel "Item I7"@en-AU ;
    dcat:accessURL <https://www.legislation.gov.au/C2004A01224/2019-02-24/2019-02-24/text/1/epub/OEBPS/document_1/document_1.html#_Toc1469127> ;
    dcat:landingPage "https://www.legislation.gov.au/C2004A01224/2019-02-24/2019-02-24/text/1/epub/OEBPS/document_1/document_1.html#_Toc1469127"^^xsd:anyURI ;
    dcat:theme legcons:Item .

C2004A01224:70 a legcons:Item,
        C2004A01224:Item,
        owl:Class,
        dcat:Resource ;
    rdfs:label "Item - I70 39  Tabling of explanatory statements"@en-AU ;
    dct:isPartOf C2004A01224:66 ;
    rdfs:comment "39  Tabling of explanatory statements - Abrievated Graph Key: I70"@en-AU ;
    rdfs:subClassOf C2004A01224: ;
    skos:definition "39  Tabling of explanatory statements"@en-AU ;
    skos:narrower C2004A01224:66 ;
    skos:prefLabel "Item I70"@en-AU ;
    dcat:accessURL <https://www.legislation.gov.au/C2004A01224/2019-02-24/2019-02-24/text/1/epub/OEBPS/document_1/document_1.html#_Toc1469190> ;
    dcat:landingPage "https://www.legislation.gov.au/C2004A01224/2019-02-24/2019-02-24/text/1/epub/OEBPS/document_1/document_1.html#_Toc1469190"^^xsd:anyURI ;
    dcat:theme legcons:Item .

C2004A01224:71 a legcons:Item,
        C2004A01224:Item,
        owl:Class,
        dcat:Resource ;
    rdfs:label "Item - I71 40  Regulations may specify manner of delivery of certain documents"@en-AU ;
    dct:isPartOf C2004A01224:66 ;
    rdfs:comment "40  Regulations may specify manner of delivery of certain documents - Abrievated Graph Key: I71"@en-AU ;
    rdfs:subClassOf C2004A01224: ;
    skos:definition "40  Regulations may specify manner of delivery of certain documents"@en-AU ;
    skos:narrower C2004A01224:66 ;
    skos:prefLabel "Item I71"@en-AU ;
    dcat:accessURL <https://www.legislation.gov.au/C2004A01224/2019-02-24/2019-02-24/text/1/epub/OEBPS/document_1/document_1.html#_Toc1469191> ;
    dcat:landingPage "https://www.legislation.gov.au/C2004A01224/2019-02-24/2019-02-24/text/1/epub/OEBPS/document_1/document_1.html#_Toc1469191"^^xsd:anyURI ;
    dcat:theme legcons:Item .

C2004A01224:72 a legcons:Item,
        C2004A01224:Item,
        owl:Class,
        dcat:Resource ;
    rdfs:label "Item - I72 41  Incorporated material may be required to be made available"@en-AU ;
    dct:isPartOf C2004A01224:66 ;
    rdfs:comment "41  Incorporated material may be required to be made available - Abrievated Graph Key: I72"@en-AU ;
    rdfs:subClassOf C2004A01224: ;
    skos:definition "41  Incorporated material may be required to be made available"@en-AU ;
    skos:narrower C2004A01224:66 ;
    skos:prefLabel "Item I72"@en-AU ;
    dcat:accessURL <https://www.legislation.gov.au/C2004A01224/2019-02-24/2019-02-24/text/1/epub/OEBPS/document_1/document_1.html#_Toc1469192> ;
    dcat:landingPage "https://www.legislation.gov.au/C2004A01224/2019-02-24/2019-02-24/text/1/epub/OEBPS/document_1/document_1.html#_Toc1469192"^^xsd:anyURI ;
    dcat:theme legcons:Item .

C2004A01224:73 a legcons:Item,
        C2004A01224:Item,
        owl:Class,
        dcat:Resource ;
    rdfs:label "Item - I73 42  Disallowance of legislative instruments"@en-AU ;
    dct:isPartOf C2004A01224:66 ;
    rdfs:comment "42  Disallowance of legislative instruments - Abrievated Graph Key: I73"@en-AU ;
    rdfs:subClassOf C2004A01224: ;
    skos:definition "42  Disallowance of legislative instruments"@en-AU ;
    skos:narrower C2004A01224:66 ;
    skos:prefLabel "Item I73"@en-AU ;
    dcat:accessURL <https://www.legislation.gov.au/C2004A01224/2019-02-24/2019-02-24/text/1/epub/OEBPS/document_1/document_1.html#_Toc1469193> ;
    dcat:landingPage "https://www.legislation.gov.au/C2004A01224/2019-02-24/2019-02-24/text/1/epub/OEBPS/document_1/document_1.html#_Toc1469193"^^xsd:anyURI ;
    dcat:theme legcons:Item .

C2004A01224:74 a legcons:Item,
        C2004A01224:Item,
        owl:Class,
        dcat:Resource ;
    rdfs:label "Item - I74 44  Legislative instruments that are not subject to disallowance"@en-AU ;
    dct:isPartOf C2004A01224:66 ;
    rdfs:comment "44  Legislative instruments that are not subject to disallowance - Abrievated Graph Key: I74"@en-AU ;
    rdfs:subClassOf C2004A01224: ;
    skos:definition "44  Legislative instruments that are not subject to disallowance"@en-AU ;
    skos:narrower C2004A01224:66 ;
    skos:prefLabel "Item I74"@en-AU ;
    dcat:accessURL <https://www.legislation.gov.au/C2004A01224/2019-02-24/2019-02-24/text/1/epub/OEBPS/document_1/document_1.html#_Toc1469194> ;
    dcat:landingPage "https://www.legislation.gov.au/C2004A01224/2019-02-24/2019-02-24/text/1/epub/OEBPS/document_1/document_1.html#_Toc1469194"^^xsd:anyURI ;
    dcat:theme legcons:Item .

C2004A01224:75 a legcons:Item,
        C2004A01224:Item,
        owl:Class,
        dcat:Resource ;
    rdfs:label "Item - I75 45  Reviving a legislative instrument law or provision"@en-AU ;
    dct:isPartOf C2004A01224:66 ;
    rdfs:comment "45  Reviving a legislative instrument law or provision - Abrievated Graph Key: I75"@en-AU ;
    rdfs:subClassOf C2004A01224: ;
    skos:definition "45  Reviving a legislative instrument law or provision"@en-AU ;
    skos:narrower C2004A01224:66 ;
    skos:prefLabel "Item I75"@en-AU ;
    dcat:accessURL <https://www.legislation.gov.au/C2004A01224/2019-02-24/2019-02-24/text/1/epub/OEBPS/document_1/document_1.html#_Toc1469195> ;
    dcat:landingPage "https://www.legislation.gov.au/C2004A01224/2019-02-24/2019-02-24/text/1/epub/OEBPS/document_1/document_1.html#_Toc1469195"^^xsd:anyURI ;
    dcat:theme legcons:Item .

C2004A01224:76 a legcons:Item,
        C2004A01224:Item,
        owl:Class,
        dcat:Resource ;
    rdfs:label "Item - I76 46  Legislative instruments not to be remade while required to be tabled"@en-AU ;
    dct:isPartOf C2004A01224:66 ;
    rdfs:comment "46  Legislative instruments not to be remade while required to be tabled - Abrievated Graph Key: I76"@en-AU ;
    rdfs:subClassOf C2004A01224: ;
    skos:definition "46  Legislative instruments not to be remade while required to be tabled"@en-AU ;
    skos:narrower C2004A01224:66 ;
    skos:prefLabel "Item I76"@en-AU ;
    dcat:accessURL <https://www.legislation.gov.au/C2004A01224/2019-02-24/2019-02-24/text/1/epub/OEBPS/document_1/document_1.html#_Toc1469196> ;
    dcat:landingPage "https://www.legislation.gov.au/C2004A01224/2019-02-24/2019-02-24/text/1/epub/OEBPS/document_1/document_1.html#_Toc1469196"^^xsd:anyURI ;
    dcat:theme legcons:Item .

C2004A01224:77 a legcons:Item,
        C2004A01224:Item,
        owl:Class,
        dcat:Resource ;
    rdfs:label "Item - I77 47  Legislative instruments not to be remade while subject to disallowance"@en-AU ;
    dct:isPartOf C2004A01224:66 ;
    rdfs:comment "47  Legislative instruments not to be remade while subject to disallowance - Abrievated Graph Key: I77"@en-AU ;
    rdfs:subClassOf C2004A01224: ;
    skos:definition "47  Legislative instruments not to be remade while subject to disallowance"@en-AU ;
    skos:narrower C2004A01224:66 ;
    skos:prefLabel "Item I77"@en-AU ;
    dcat:accessURL <https://www.legislation.gov.au/C2004A01224/2019-02-24/2019-02-24/text/1/epub/OEBPS/document_1/document_1.html#_Toc1469197> ;
    dcat:landingPage "https://www.legislation.gov.au/C2004A01224/2019-02-24/2019-02-24/text/1/epub/OEBPS/document_1/document_1.html#_Toc1469197"^^xsd:anyURI ;
    dcat:theme legcons:Item .

C2004A01224:78 a legcons:Item,
        C2004A01224:Item,
        owl:Class,
        dcat:Resource ;
    rdfs:label "Item - I78 48  Remaking disallowed legislative instruments"@en-AU ;
    dct:isPartOf C2004A01224:66 ;
    rdfs:comment "48  Remaking disallowed legislative instruments - Abrievated Graph Key: I78"@en-AU ;
    rdfs:subClassOf C2004A01224: ;
    skos:definition "48  Remaking disallowed legislative instruments"@en-AU ;
    skos:narrower C2004A01224:66 ;
    skos:prefLabel "Item I78"@en-AU ;
    dcat:accessURL <https://www.legislation.gov.au/C2004A01224/2019-02-24/2019-02-24/text/1/epub/OEBPS/document_1/document_1.html#_Toc1469198> ;
    dcat:landingPage "https://www.legislation.gov.au/C2004A01224/2019-02-24/2019-02-24/text/1/epub/OEBPS/document_1/document_1.html#_Toc1469198"^^xsd:anyURI ;
    dcat:theme legcons:Item .

C2004A01224:8 a legcons:Item,
        C2004A01224:Item,
        owl:Class,
        dcat:Resource ;
    rdfs:label "Item - I8 4  The Dictionary"@en-AU ;
    dct:isPartOf C2004A01224:1 ;
    rdfs:comment "4  The Dictionary - Abrievated Graph Key: I8"@en-AU ;
    rdfs:subClassOf C2004A01224: ;
    skos:definition "4  The Dictionary"@en-AU ;
    skos:narrower C2004A01224:1 ;
    skos:prefLabel "Item I8"@en-AU ;
    dcat:accessURL <https://www.legislation.gov.au/C2004A01224/2019-02-24/2019-02-24/text/1/epub/OEBPS/document_1/document_1.html#_Toc1469128> ;
    dcat:landingPage "https://www.legislation.gov.au/C2004A01224/2019-02-24/2019-02-24/text/1/epub/OEBPS/document_1/document_1.html#_Toc1469128"^^xsd:anyURI ;
    dcat:theme legcons:Item .

C2004A01224:81 a legcons:Item,
        C2004A01224:Item,
        owl:Class,
        dcat:Resource ;
    rdfs:label "Item - I81 48 AA  Simplified outline of this Part"@en-AU ;
    dct:isPartOf C2004A01224:80 ;
    rdfs:comment "48 AA  Simplified outline of this Part - Abrievated Graph Key: I81"@en-AU ;
    rdfs:subClassOf C2004A01224: ;
    skos:definition "48 AA  Simplified outline of this Part"@en-AU ;
    skos:narrower C2004A01224:80 ;
    skos:prefLabel "Item I81"@en-AU ;
    dcat:accessURL <https://www.legislation.gov.au/C2004A01224/2019-02-24/2019-02-24/text/1/epub/OEBPS/document_1/document_1.html#_Toc1469201> ;
    dcat:landingPage "https://www.legislation.gov.au/C2004A01224/2019-02-24/2019-02-24/text/1/epub/OEBPS/document_1/document_1.html#_Toc1469201"^^xsd:anyURI ;
    dcat:theme legcons:Item .

C2004A01224:84 a legcons:Item,
        C2004A01224:Item,
        owl:Class,
        dcat:Resource ;
    rdfs:label "Item - I84 48 A  Automatic repeal of amending and repealing instruments"@en-AU ;
    dct:isPartOf C2004A01224:83 ;
    rdfs:comment "48 A  Automatic repeal of amending and repealing instruments - Abrievated Graph Key: I84"@en-AU ;
    rdfs:subClassOf C2004A01224: ;
    skos:definition "48 A  Automatic repeal of amending and repealing instruments"@en-AU ;
    skos:narrower C2004A01224:83 ;
    skos:prefLabel "Item I84"@en-AU ;
    dcat:accessURL <https://www.legislation.gov.au/C2004A01224/2019-02-24/2019-02-24/text/1/epub/OEBPS/document_1/document_1.html#_Toc1469204> ;
    dcat:landingPage "https://www.legislation.gov.au/C2004A01224/2019-02-24/2019-02-24/text/1/epub/OEBPS/document_1/document_1.html#_Toc1469204"^^xsd:anyURI ;
    dcat:theme legcons:Item .

C2004A01224:85 a legcons:Subdivision,
        C2004A01224:Subdivision,
        owl:Class,
        dcat:Resource ;
    rdfs:label "Subdivision - S85 Subdivision BRepeal of commencement instruments"@en-AU ;
    dct:isPartOf C2004A01224:82 ;
    rdfs:comment "Subdivision BRepeal of commencement instruments - Abrievated Graph Key: S85"@en-AU ;
    rdfs:subClassOf C2004A01224: ;
    skos:definition "Subdivision BRepeal of commencement instruments"@en-AU ;
    skos:narrower C2004A01224:82 ;
    skos:prefLabel "Subdivision S85"@en-AU ;
    dcat:accessURL <https://www.legislation.gov.au/C2004A01224/2019-02-24/2019-02-24/text/1/epub/OEBPS/document_1/document_1.html#_Toc1469205> ;
    dcat:landingPage "https://www.legislation.gov.au/C2004A01224/2019-02-24/2019-02-24/text/1/epub/OEBPS/document_1/document_1.html#_Toc1469205"^^xsd:anyURI ;
    dcat:theme legcons:Subdivision .

C2004A01224:86 a legcons:Item,
        C2004A01224:Item,
        owl:Class,
        dcat:Resource ;
    rdfs:label "Item - I86 48 B  Automatic repeal of commencement instruments"@en-AU ;
    dct:isPartOf C2004A01224:82 ;
    rdfs:comment "48 B  Automatic repeal of commencement instruments - Abrievated Graph Key: I86"@en-AU ;
    rdfs:subClassOf C2004A01224: ;
    skos:definition "48 B  Automatic repeal of commencement instruments"@en-AU ;
    skos:narrower C2004A01224:82 ;
    skos:prefLabel "Item I86"@en-AU ;
    dcat:accessURL <https://www.legislation.gov.au/C2004A01224/2019-02-24/2019-02-24/text/1/epub/OEBPS/document_1/document_1.html#_Toc1469206> ;
    dcat:landingPage "https://www.legislation.gov.au/C2004A01224/2019-02-24/2019-02-24/text/1/epub/OEBPS/document_1/document_1.html#_Toc1469206"^^xsd:anyURI ;
    dcat:theme legcons:Item .

C2004A01224:87 a legcons:Subdivision,
        C2004A01224:Subdivision,
        owl:Class,
        dcat:Resource ;
    rdfs:label "Subdivision - S87 Subdivision CRepeal of amending or repealing provisions of instruments containing other matter"@en-AU ;
    dct:isPartOf C2004A01224:82 ;
    rdfs:comment "Subdivision CRepeal of amending or repealing provisions of instruments containing other matter - Abrievated Graph Key: S87"@en-AU ;
    rdfs:subClassOf C2004A01224: ;
    skos:definition "Subdivision CRepeal of amending or repealing provisions of instruments containing other matter"@en-AU ;
    skos:narrower C2004A01224:82 ;
    skos:prefLabel "Subdivision S87"@en-AU ;
    dcat:accessURL <https://www.legislation.gov.au/C2004A01224/2019-02-24/2019-02-24/text/1/epub/OEBPS/document_1/document_1.html#_Toc1469207> ;
    dcat:landingPage "https://www.legislation.gov.au/C2004A01224/2019-02-24/2019-02-24/text/1/epub/OEBPS/document_1/document_1.html#_Toc1469207"^^xsd:anyURI ;
    dcat:theme legcons:Subdivision .

C2004A01224:88 a legcons:Item,
        C2004A01224:Item,
        owl:Class,
        dcat:Resource ;
    rdfs:label "Item - I88 48 C  Automatic repeal of amending and repealing provisions"@en-AU ;
    dct:isPartOf C2004A01224:82 ;
    rdfs:comment "48 C  Automatic repeal of amending and repealing provisions - Abrievated Graph Key: I88"@en-AU ;
    rdfs:subClassOf C2004A01224: ;
    skos:definition "48 C  Automatic repeal of amending and repealing provisions"@en-AU ;
    skos:narrower C2004A01224:82 ;
    skos:prefLabel "Item I88"@en-AU ;
    dcat:accessURL <https://www.legislation.gov.au/C2004A01224/2019-02-24/2019-02-24/text/1/epub/OEBPS/document_1/document_1.html#_Toc1469208> ;
    dcat:landingPage "https://www.legislation.gov.au/C2004A01224/2019-02-24/2019-02-24/text/1/epub/OEBPS/document_1/document_1.html#_Toc1469208"^^xsd:anyURI ;
    dcat:theme legcons:Item .

C2004A01224:89 a legcons:Subdivision,
        C2004A01224:Subdivision,
        owl:Class,
        dcat:Resource ;
    rdfs:label "Subdivision - S89 Subdivision DRepeal of commencement provisions of instruments containing other matter"@en-AU ;
    dct:isPartOf C2004A01224:82 ;
    rdfs:comment "Subdivision DRepeal of commencement provisions of instruments containing other matter - Abrievated Graph Key: S89"@en-AU ;
    rdfs:subClassOf C2004A01224: ;
    skos:definition "Subdivision DRepeal of commencement provisions of instruments containing other matter"@en-AU ;
    skos:narrower C2004A01224:82 ;
    skos:prefLabel "Subdivision S89"@en-AU ;
    dcat:accessURL <https://www.legislation.gov.au/C2004A01224/2019-02-24/2019-02-24/text/1/epub/OEBPS/document_1/document_1.html#_Toc1469209> ;
    dcat:landingPage "https://www.legislation.gov.au/C2004A01224/2019-02-24/2019-02-24/text/1/epub/OEBPS/document_1/document_1.html#_Toc1469209"^^xsd:anyURI ;
    dcat:theme legcons:Subdivision .

C2004A01224:9 a legcons:Item,
        C2004A01224:Item,
        owl:Class,
        dcat:Resource ;
    rdfs:label "Item - I9 5  Definitions of amend and modify"@en-AU ;
    dct:isPartOf C2004A01224:1 ;
    rdfs:comment "5  Definitions of amend and modify - Abrievated Graph Key: I9"@en-AU ;
    rdfs:subClassOf C2004A01224: ;
    skos:definition "5  Definitions of amend and modify"@en-AU ;
    skos:narrower C2004A01224:1 ;
    skos:prefLabel "Item I9"@en-AU ;
    dcat:accessURL <https://www.legislation.gov.au/C2004A01224/2019-02-24/2019-02-24/text/1/epub/OEBPS/document_1/document_1.html#_Toc1469129> ;
    dcat:landingPage "https://www.legislation.gov.au/C2004A01224/2019-02-24/2019-02-24/text/1/epub/OEBPS/document_1/document_1.html#_Toc1469129"^^xsd:anyURI ;
    dcat:theme legcons:Item .

C2004A01224:90 a legcons:Item,
        C2004A01224:Item,
        owl:Class,
        dcat:Resource ;
    rdfs:label "Item - I90 48 D  Automatic repeal of commencement provisions"@en-AU ;
    dct:isPartOf C2004A01224:82 ;
    rdfs:comment "48 D  Automatic repeal of commencement provisions - Abrievated Graph Key: I90"@en-AU ;
    rdfs:subClassOf C2004A01224: ;
    skos:definition "48 D  Automatic repeal of commencement provisions"@en-AU ;
    skos:narrower C2004A01224:82 ;
    skos:prefLabel "Item I90"@en-AU ;
    dcat:accessURL <https://www.legislation.gov.au/C2004A01224/2019-02-24/2019-02-24/text/1/epub/OEBPS/document_1/document_1.html#_Toc1469210> ;
    dcat:landingPage "https://www.legislation.gov.au/C2004A01224/2019-02-24/2019-02-24/text/1/epub/OEBPS/document_1/document_1.html#_Toc1469210"^^xsd:anyURI ;
    dcat:theme legcons:Item .

C2004A01224:91 a legcons:Division,
        C2004A01224:Division,
        owl:Class,
        dcat:Resource ;
    rdfs:label "Division - D91 Division 2 Repeal by regulations"@en-AU ;
    dct:isPartOf C2004A01224:79 ;
    rdfs:comment "Division 2 Repeal by regulations - Abrievated Graph Key: D91"@en-AU ;
    rdfs:subClassOf C2004A01224: ;
    skos:definition "Division 2 Repeal by regulations"@en-AU ;
    skos:narrower C2004A01224:79 ;
    skos:prefLabel "Division D91"@en-AU ;
    dcat:accessURL <https://www.legislation.gov.au/C2004A01224/2019-02-24/2019-02-24/text/1/epub/OEBPS/document_1/document_1.html#_Toc1469211> ;
    dcat:landingPage "https://www.legislation.gov.au/C2004A01224/2019-02-24/2019-02-24/text/1/epub/OEBPS/document_1/document_1.html#_Toc1469211"^^xsd:anyURI ;
    dcat:theme legcons:Division .

C2004A01224:92 a legcons:Item,
        C2004A01224:Item,
        owl:Class,
        dcat:Resource ;
    rdfs:label "Item - I92 48 E  Regulations may repeal instruments or provisions no longer required"@en-AU ;
    dct:isPartOf C2004A01224:79 ;
    rdfs:comment "48 E  Regulations may repeal instruments or provisions no longer required - Abrievated Graph Key: I92"@en-AU ;
    rdfs:subClassOf C2004A01224: ;
    skos:definition "48 E  Regulations may repeal instruments or provisions no longer required"@en-AU ;
    skos:narrower C2004A01224:79 ;
    skos:prefLabel "Item I92"@en-AU ;
    dcat:accessURL <https://www.legislation.gov.au/C2004A01224/2019-02-24/2019-02-24/text/1/epub/OEBPS/document_1/document_1.html#_Toc1469212> ;
    dcat:landingPage "https://www.legislation.gov.au/C2004A01224/2019-02-24/2019-02-24/text/1/epub/OEBPS/document_1/document_1.html#_Toc1469212"^^xsd:anyURI ;
    dcat:theme legcons:Item .

C2004A01224:93 a legcons:Part,
        C2004A01224:Part,
        owl:Class,
        dcat:Resource ;
    rdfs:label "Part - P93 Part 4 Sunsetting of legislative instruments"@en-AU ;
    dct:isPartOf C2004A01224:60 ;
    rdfs:comment "Part 4 Sunsetting of legislative instruments - Abrievated Graph Key: P93"@en-AU ;
    rdfs:subClassOf C2004A01224: ;
    skos:definition "Part 4 Sunsetting of legislative instruments"@en-AU ;
    skos:narrower C2004A01224:60 ;
    skos:prefLabel "Part P93"@en-AU ;
    dcat:accessURL <https://www.legislation.gov.au/C2004A01224/2019-02-24/2019-02-24/text/1/epub/OEBPS/document_1/document_1.html#_Toc1469213> ;
    dcat:landingPage "https://www.legislation.gov.au/C2004A01224/2019-02-24/2019-02-24/text/1/epub/OEBPS/document_1/document_1.html#_Toc1469213"^^xsd:anyURI ;
    dcat:theme legcons:Part .

C2004A01224:94 a legcons:Item,
        C2004A01224:Item,
        owl:Class,
        dcat:Resource ;
    rdfs:label "Item - I94 48 F  Simplified outline of this Part"@en-AU ;
    dct:isPartOf C2004A01224:60 ;
    rdfs:comment "48 F  Simplified outline of this Part - Abrievated Graph Key: I94"@en-AU ;
    rdfs:subClassOf C2004A01224: ;
    skos:definition "48 F  Simplified outline of this Part"@en-AU ;
    skos:narrower C2004A01224:60 ;
    skos:prefLabel "Item I94"@en-AU ;
    dcat:accessURL <https://www.legislation.gov.au/C2004A01224/2019-02-24/2019-02-24/text/1/epub/OEBPS/document_1/document_1.html#_Toc1469214> ;
    dcat:landingPage "https://www.legislation.gov.au/C2004A01224/2019-02-24/2019-02-24/text/1/epub/OEBPS/document_1/document_1.html#_Toc1469214"^^xsd:anyURI ;
    dcat:theme legcons:Item .

C2004A01224:95 a legcons:Item,
        C2004A01224:Item,
        owl:Class,
        dcat:Resource ;
    rdfs:label "Item - I95 49  The purpose of the Part"@en-AU ;
    dct:isPartOf C2004A01224:60 ;
    rdfs:comment "49  The purpose of the Part - Abrievated Graph Key: I95"@en-AU ;
    rdfs:subClassOf C2004A01224: ;
    skos:definition "49  The purpose of the Part"@en-AU ;
    skos:narrower C2004A01224:60 ;
    skos:prefLabel "Item I95"@en-AU ;
    dcat:accessURL <https://www.legislation.gov.au/C2004A01224/2019-02-24/2019-02-24/text/1/epub/OEBPS/document_1/document_1.html#_Toc1469215> ;
    dcat:landingPage "https://www.legislation.gov.au/C2004A01224/2019-02-24/2019-02-24/text/1/epub/OEBPS/document_1/document_1.html#_Toc1469215"^^xsd:anyURI ;
    dcat:theme legcons:Item .

C2004A01224:96 a legcons:Item,
        C2004A01224:Item,
        owl:Class,
        dcat:Resource ;
    rdfs:label "Item - I96 50  Sunsetting"@en-AU ;
    dct:isPartOf C2004A01224:60 ;
    rdfs:comment "50  Sunsetting - Abrievated Graph Key: I96"@en-AU ;
    rdfs:subClassOf C2004A01224: ;
    skos:definition "50  Sunsetting"@en-AU ;
    skos:narrower C2004A01224:60 ;
    skos:prefLabel "Item I96"@en-AU ;
    dcat:accessURL <https://www.legislation.gov.au/C2004A01224/2019-02-24/2019-02-24/text/1/epub/OEBPS/document_1/document_1.html#_Toc1469216> ;
    dcat:landingPage "https://www.legislation.gov.au/C2004A01224/2019-02-24/2019-02-24/text/1/epub/OEBPS/document_1/document_1.html#_Toc1469216"^^xsd:anyURI ;
    dcat:theme legcons:Item .

C2004A01224:97 a legcons:Item,
        C2004A01224:Item,
        owl:Class,
        dcat:Resource ;
    rdfs:label "Item - I97 51  Attorney General may defer sunsetting in certain circumstances"@en-AU ;
    dct:isPartOf C2004A01224:60 ;
    rdfs:comment "51  Attorney General may defer sunsetting in certain circumstances - Abrievated Graph Key: I97"@en-AU ;
    rdfs:subClassOf C2004A01224: ;
    skos:definition "51  Attorney General may defer sunsetting in certain circumstances"@en-AU ;
    skos:narrower C2004A01224:60 ;
    skos:prefLabel "Item I97"@en-AU ;
    dcat:accessURL <https://www.legislation.gov.au/C2004A01224/2019-02-24/2019-02-24/text/1/epub/OEBPS/document_1/document_1.html#_Toc1469217> ;
    dcat:landingPage "https://www.legislation.gov.au/C2004A01224/2019-02-24/2019-02-24/text/1/epub/OEBPS/document_1/document_1.html#_Toc1469217"^^xsd:anyURI ;
    dcat:theme legcons:Item .

C2004A01224:98 a legcons:Item,
        C2004A01224:Item,
        owl:Class,
        dcat:Resource ;
    rdfs:label "Item - I98 51 A  Attorney General may align sunsetting of instruments to be reviewed together"@en-AU ;
    dct:isPartOf C2004A01224:60 ;
    rdfs:comment "51 A  Attorney General may align sunsetting of instruments to be reviewed together - Abrievated Graph Key: I98"@en-AU ;
    rdfs:subClassOf C2004A01224: ;
    skos:definition "51 A  Attorney General may align sunsetting of instruments to be reviewed together"@en-AU ;
    skos:narrower C2004A01224:60 ;
    skos:prefLabel "Item I98"@en-AU ;
    dcat:accessURL <https://www.legislation.gov.au/C2004A01224/2019-02-24/2019-02-24/text/1/epub/OEBPS/document_1/document_1.html#_Toc1469218> ;
    dcat:landingPage "https://www.legislation.gov.au/C2004A01224/2019-02-24/2019-02-24/text/1/epub/OEBPS/document_1/document_1.html#_Toc1469218"^^xsd:anyURI ;
    dcat:theme legcons:Item .

C2004A01224:99 a legcons:Item,
        C2004A01224:Item,
        owl:Class,
        dcat:Resource ;
    rdfs:label "Item - I99 52  Attorney General must lay lists of instruments due for sunsetting before each House of the Parliament"@en-AU ;
    dct:isPartOf C2004A01224:60 ;
    rdfs:comment "52  Attorney General must lay lists of instruments due for sunsetting before each House of the Parliament - Abrievated Graph Key: I99"@en-AU ;
    rdfs:subClassOf C2004A01224: ;
    skos:definition "52  Attorney General must lay lists of instruments due for sunsetting before each House of the Parliament"@en-AU ;
    skos:narrower C2004A01224:60 ;
    skos:prefLabel "Item I99"@en-AU ;
    dcat:accessURL <https://www.legislation.gov.au/C2004A01224/2019-02-24/2019-02-24/text/1/epub/OEBPS/document_1/document_1.html#_Toc1469219> ;
    dcat:landingPage "https://www.legislation.gov.au/C2004A01224/2019-02-24/2019-02-24/text/1/epub/OEBPS/document_1/document_1.html#_Toc1469219"^^xsd:anyURI ;
    dcat:theme legcons:Item .

C2004A01224:22 a legcons:Division,
        C2004A01224:Division,
        owl:Class,
        dcat:Resource ;
    rdfs:label "Division - D22 Division 1 Simplified outline of this Part"@en-AU ;
    dct:hasPart C2004A01224:23 ;
    dct:isPartOf C2004A01224:21 ;
    rdfs:comment "Division 1 Simplified outline of this Part - Abrievated Graph Key: D22"@en-AU ;
    rdfs:subClassOf C2004A01224: ;
    skos:broader C2004A01224:23 ;
    skos:definition "Division 1 Simplified outline of this Part"@en-AU ;
    skos:narrower C2004A01224:21 ;
    skos:prefLabel "Division D22"@en-AU ;
    dcat:accessURL <https://www.legislation.gov.au/C2004A01224/2019-02-24/2019-02-24/text/1/epub/OEBPS/document_1/document_1.html#_Toc1469142> ;
    dcat:landingPage "https://www.legislation.gov.au/C2004A01224/2019-02-24/2019-02-24/text/1/epub/OEBPS/document_1/document_1.html#_Toc1469142"^^xsd:anyURI ;
    dcat:theme legcons:Division .

C2004A01224:40 a legcons:Division,
        C2004A01224:Division,
        owl:Class,
        dcat:Resource ;
    rdfs:label "Division - D40 Division 1 Simplified outline of this Part"@en-AU ;
    dct:hasPart C2004A01224:41 ;
    dct:isPartOf C2004A01224:20 ;
    rdfs:comment "Division 1 Simplified outline of this Part - Abrievated Graph Key: D40"@en-AU ;
    rdfs:subClassOf C2004A01224: ;
    skos:broader C2004A01224:41 ;
    skos:definition "Division 1 Simplified outline of this Part"@en-AU ;
    skos:narrower C2004A01224:20 ;
    skos:prefLabel "Division D40"@en-AU ;
    dcat:accessURL <https://www.legislation.gov.au/C2004A01224/2019-02-24/2019-02-24/text/1/epub/OEBPS/document_1/document_1.html#_Toc1469160> ;
    dcat:landingPage "https://www.legislation.gov.au/C2004A01224/2019-02-24/2019-02-24/text/1/epub/OEBPS/document_1/document_1.html#_Toc1469160"^^xsd:anyURI ;
    dcat:theme legcons:Division .

C2004A01224:80 a legcons:Division,
        C2004A01224:Division,
        owl:Class,
        dcat:Resource ;
    rdfs:label "Division - D80 Division 1 ASimplified outline of this Part"@en-AU ;
    dct:hasPart C2004A01224:81 ;
    dct:isPartOf C2004A01224:79 ;
    rdfs:comment "Division 1 ASimplified outline of this Part - Abrievated Graph Key: D80"@en-AU ;
    rdfs:subClassOf C2004A01224: ;
    skos:broader C2004A01224:81 ;
    skos:definition "Division 1 ASimplified outline of this Part"@en-AU ;
    skos:narrower C2004A01224:79 ;
    skos:prefLabel "Division D80"@en-AU ;
    dcat:accessURL <https://www.legislation.gov.au/C2004A01224/2019-02-24/2019-02-24/text/1/epub/OEBPS/document_1/document_1.html#_Toc1469200> ;
    dcat:landingPage "https://www.legislation.gov.au/C2004A01224/2019-02-24/2019-02-24/text/1/epub/OEBPS/document_1/document_1.html#_Toc1469200"^^xsd:anyURI ;
    dcat:theme legcons:Division .

C2004A01224:83 a legcons:Subdivision,
        C2004A01224:Subdivision,
        owl:Class,
        dcat:Resource ;
    rdfs:label "Subdivision - S83 Subdivision ARepeal of amending and repealing instruments"@en-AU ;
    dct:hasPart C2004A01224:84 ;
    dct:isPartOf C2004A01224:82 ;
    rdfs:comment "Subdivision ARepeal of amending and repealing instruments - Abrievated Graph Key: S83"@en-AU ;
    rdfs:subClassOf C2004A01224: ;
    skos:broader C2004A01224:84 ;
    skos:definition "Subdivision ARepeal of amending and repealing instruments"@en-AU ;
    skos:narrower C2004A01224:82 ;
    skos:prefLabel "Subdivision S83"@en-AU ;
    dcat:accessURL <https://www.legislation.gov.au/C2004A01224/2019-02-24/2019-02-24/text/1/epub/OEBPS/document_1/document_1.html#_Toc1469203> ;
    dcat:landingPage "https://www.legislation.gov.au/C2004A01224/2019-02-24/2019-02-24/text/1/epub/OEBPS/document_1/document_1.html#_Toc1469203"^^xsd:anyURI ;
    dcat:theme legcons:Subdivision .

C2004A01224:54 a legcons:Division,
        C2004A01224:Division,
        owl:Class,
        dcat:Resource ;
    rdfs:label "Division - D54 Division 1 Introduction"@en-AU ;
    dct:hasPart C2004A01224:55,
        C2004A01224:56 ;
    dct:isPartOf C2004A01224:20 ;
    rdfs:comment "Division 1 Introduction - Abrievated Graph Key: D54"@en-AU ;
    rdfs:subClassOf C2004A01224: ;
    skos:broader C2004A01224:55,
        C2004A01224:56 ;
    skos:definition "Division 1 Introduction"@en-AU ;
    skos:narrower C2004A01224:20 ;
    skos:prefLabel "Division D54"@en-AU ;
    dcat:accessURL <https://www.legislation.gov.au/C2004A01224/2019-02-24/2019-02-24/text/1/epub/OEBPS/document_1/document_1.html#_Toc1469174> ;
    dcat:landingPage "https://www.legislation.gov.au/C2004A01224/2019-02-24/2019-02-24/text/1/epub/OEBPS/document_1/document_1.html#_Toc1469174"^^xsd:anyURI ;
    dcat:theme legcons:Division .

C2004A01224:57 a legcons:Division,
        C2004A01224:Division,
        owl:Class,
        dcat:Resource ;
    rdfs:label "Division - D57 Division 2 Authorised versions and judicial notice"@en-AU ;
    dct:hasPart C2004A01224:58,
        C2004A01224:59 ;
    dct:isPartOf C2004A01224:20 ;
    rdfs:comment "Division 2 Authorised versions and judicial notice - Abrievated Graph Key: D57"@en-AU ;
    rdfs:subClassOf C2004A01224: ;
    skos:broader C2004A01224:58,
        C2004A01224:59 ;
    skos:definition "Division 2 Authorised versions and judicial notice"@en-AU ;
    skos:narrower C2004A01224:20 ;
    skos:prefLabel "Division D57"@en-AU ;
    dcat:accessURL <https://www.legislation.gov.au/C2004A01224/2019-02-24/2019-02-24/text/1/epub/OEBPS/document_1/document_1.html#_Toc1469177> ;
    dcat:landingPage "https://www.legislation.gov.au/C2004A01224/2019-02-24/2019-02-24/text/1/epub/OEBPS/document_1/document_1.html#_Toc1469177"^^xsd:anyURI ;
    dcat:theme legcons:Division .

C2004A01224:49 a legcons:Division,
        C2004A01224:Division,
        owl:Class,
        dcat:Resource ;
    rdfs:label "Division - D49 Division 3 Editorial changes and other changes"@en-AU ;
    dct:hasPart C2004A01224:50,
        C2004A01224:51,
        C2004A01224:52 ;
    dct:isPartOf C2004A01224:20 ;
    rdfs:comment "Division 3 Editorial changes and other changes - Abrievated Graph Key: D49"@en-AU ;
    rdfs:subClassOf C2004A01224: ;
    skos:broader C2004A01224:50,
        C2004A01224:51,
        C2004A01224:52 ;
    skos:definition "Division 3 Editorial changes and other changes"@en-AU ;
    skos:narrower C2004A01224:20 ;
    skos:prefLabel "Division D49"@en-AU ;
    dcat:accessURL <https://www.legislation.gov.au/C2004A01224/2019-02-24/2019-02-24/text/1/epub/OEBPS/document_1/document_1.html#_Toc1469169> ;
    dcat:landingPage "https://www.legislation.gov.au/C2004A01224/2019-02-24/2019-02-24/text/1/epub/OEBPS/document_1/document_1.html#_Toc1469169"^^xsd:anyURI ;
    dcat:theme legcons:Division .

C2004A01224:61 a legcons:Part,
        C2004A01224:Part,
        owl:Class,
        dcat:Resource ;
    rdfs:label "Part - P61 Part 1 Drafting standards and consultation"@en-AU ;
    dct:hasPart C2004A01224:62,
        C2004A01224:63,
        C2004A01224:64,
        C2004A01224:65 ;
    dct:isPartOf C2004A01224:60 ;
    rdfs:comment "Part 1 Drafting standards and consultation - Abrievated Graph Key: P61"@en-AU ;
    rdfs:subClassOf C2004A01224: ;
    skos:broader C2004A01224:62,
        C2004A01224:63,
        C2004A01224:64,
        C2004A01224:65 ;
    skos:definition "Part 1 Drafting standards and consultation"@en-AU ;
    skos:narrower C2004A01224:60 ;
    skos:prefLabel "Part P61"@en-AU ;
    dcat:accessURL <https://www.legislation.gov.au/C2004A01224/2019-02-24/2019-02-24/text/1/epub/OEBPS/document_1/document_1.html#_Toc1469181> ;
    dcat:landingPage "https://www.legislation.gov.au/C2004A01224/2019-02-24/2019-02-24/text/1/epub/OEBPS/document_1/document_1.html#_Toc1469181"^^xsd:anyURI ;
    dcat:theme legcons:Part .

C2004A01224:79 a legcons:Part,
        C2004A01224:Part,
        owl:Class,
        dcat:Resource ;
    rdfs:label "Part - P79 Part 3 Repeal of spent legislative instruments notifiable instruments and provisions"@en-AU ;
    dct:hasPart C2004A01224:80,
        C2004A01224:82,
        C2004A01224:91,
        C2004A01224:92 ;
    dct:isPartOf C2004A01224:60 ;
    rdfs:comment "Part 3 Repeal of spent legislative instruments notifiable instruments and provisions - Abrievated Graph Key: P79"@en-AU ;
    rdfs:subClassOf C2004A01224: ;
    skos:broader C2004A01224:80,
        C2004A01224:82,
        C2004A01224:91,
        C2004A01224:92 ;
    skos:definition "Part 3 Repeal of spent legislative instruments notifiable instruments and provisions"@en-AU ;
    skos:narrower C2004A01224:60 ;
    skos:prefLabel "Part P79"@en-AU ;
    dcat:accessURL <https://www.legislation.gov.au/C2004A01224/2019-02-24/2019-02-24/text/1/epub/OEBPS/document_1/document_1.html#_Toc1469199> ;
    dcat:landingPage "https://www.legislation.gov.au/C2004A01224/2019-02-24/2019-02-24/text/1/epub/OEBPS/document_1/document_1.html#_Toc1469199"^^xsd:anyURI ;
    dcat:theme legcons:Part .

C2004A01224:113 a legcons:Endnotes,
        C2004A01224:Endnotes,
        owl:Class,
        dcat:Resource ;
    rdfs:label "Endnotes - E113 Endnotes"@en-AU ;
    dct:hasPart C2004A01224:114,
        C2004A01224:115,
        C2004A01224:116,
        C2004A01224:117,
        C2004A01224:118 ;
    dct:isPartOf C2004A01224:102 ;
    rdfs:comment "Endnotes - Abrievated Graph Key: E113"@en-AU ;
    rdfs:subClassOf C2004A01224: ;
    skos:broader C2004A01224:114,
        C2004A01224:115,
        C2004A01224:116,
        C2004A01224:117,
        C2004A01224:118 ;
    skos:definition "Endnotes"@en-AU ;
    skos:narrower C2004A01224:102 ;
    skos:prefLabel "Endnotes E113"@en-AU ;
    dcat:accessURL <https://www.legislation.gov.au/C2004A01224/2019-02-24/2019-02-24/text/1/epub/OEBPS/document_1/document_1.html#_Toc1469233> ;
    dcat:landingPage "https://www.legislation.gov.au/C2004A01224/2019-02-24/2019-02-24/text/1/epub/OEBPS/document_1/document_1.html#_Toc1469233"^^xsd:anyURI ;
    dcat:theme legcons:Endnotes .

C2004A01224:42 a legcons:Division,
        C2004A01224:Division,
        owl:Class,
        dcat:Resource ;
    rdfs:label "Division - D42 Division 2 Registration of compilations"@en-AU ;
    dct:hasPart C2004A01224:43,
        C2004A01224:44,
        C2004A01224:45,
        C2004A01224:46,
        C2004A01224:47,
        C2004A01224:48 ;
    dct:isPartOf C2004A01224:20 ;
    rdfs:comment "Division 2 Registration of compilations - Abrievated Graph Key: D42"@en-AU ;
    rdfs:subClassOf C2004A01224: ;
    skos:broader C2004A01224:43,
        C2004A01224:44,
        C2004A01224:45,
        C2004A01224:46,
        C2004A01224:47,
        C2004A01224:48 ;
    skos:definition "Division 2 Registration of compilations"@en-AU ;
    skos:narrower C2004A01224:20 ;
    skos:prefLabel "Division D42"@en-AU ;
    dcat:accessURL <https://www.legislation.gov.au/C2004A01224/2019-02-24/2019-02-24/text/1/epub/OEBPS/document_1/document_1.html#_Toc1469162> ;
    dcat:landingPage "https://www.legislation.gov.au/C2004A01224/2019-02-24/2019-02-24/text/1/epub/OEBPS/document_1/document_1.html#_Toc1469162"^^xsd:anyURI ;
    dcat:theme legcons:Division .

C2004A01224:20 a legcons:Chapter,
        C2004A01224:Chapter,
        owl:Class,
        dcat:Resource ;
    rdfs:label "Chapter - C20 Chapter 2 Registration of Acts legislative instruments and notifiable instruments"@en-AU ;
    dct:hasPart C2004A01224:21,
        C2004A01224:39,
        C2004A01224:40,
        C2004A01224:42,
        C2004A01224:49,
        C2004A01224:53,
        C2004A01224:54,
        C2004A01224:57 ;
    rdfs:comment "Chapter 2 Registration of Acts legislative instruments and notifiable instruments - Abrievated Graph Key: C20"@en-AU ;
    rdfs:subClassOf C2004A01224: ;
    skos:broader C2004A01224:21,
        C2004A01224:39,
        C2004A01224:40,
        C2004A01224:42,
        C2004A01224:49,
        C2004A01224:53,
        C2004A01224:54,
        C2004A01224:57 ;
    skos:definition "Chapter 2 Registration of Acts legislative instruments and notifiable instruments"@en-AU ;
    skos:prefLabel "Chapter C20"@en-AU ;
    dcat:accessURL <https://www.legislation.gov.au/C2004A01224/2019-02-24/2019-02-24/text/1/epub/OEBPS/document_1/document_1.html#_Toc1469140> ;
    dcat:landingPage "https://www.legislation.gov.au/C2004A01224/2019-02-24/2019-02-24/text/1/epub/OEBPS/document_1/document_1.html#_Toc1469140"^^xsd:anyURI ;
    dcat:theme legcons:Chapter .

C2004A01224:82 a legcons:Division,
        C2004A01224:Division,
        owl:Class,
        dcat:Resource ;
    rdfs:label "Division - D82 Division 1 Automatic repeal"@en-AU ;
    dct:hasPart C2004A01224:83,
        C2004A01224:85,
        C2004A01224:86,
        C2004A01224:87,
        C2004A01224:88,
        C2004A01224:89,
        C2004A01224:90 ;
    dct:isPartOf C2004A01224:79 ;
    rdfs:comment "Division 1 Automatic repeal - Abrievated Graph Key: D82"@en-AU ;
    rdfs:subClassOf C2004A01224: ;
    skos:broader C2004A01224:83,
        C2004A01224:85,
        C2004A01224:86,
        C2004A01224:87,
        C2004A01224:88,
        C2004A01224:89,
        C2004A01224:90 ;
    skos:definition "Division 1 Automatic repeal"@en-AU ;
    skos:narrower C2004A01224:79 ;
    skos:prefLabel "Division D82"@en-AU ;
    dcat:accessURL <https://www.legislation.gov.au/C2004A01224/2019-02-24/2019-02-24/text/1/epub/OEBPS/document_1/document_1.html#_Toc1469202> ;
    dcat:landingPage "https://www.legislation.gov.au/C2004A01224/2019-02-24/2019-02-24/text/1/epub/OEBPS/document_1/document_1.html#_Toc1469202"^^xsd:anyURI ;
    dcat:theme legcons:Division .

C2004A01224:102 a legcons:Chapter,
        C2004A01224:Chapter,
        owl:Class,
        dcat:Resource ;
    rdfs:label "Chapter - C102 Chapter 4 Miscellaneous"@en-AU ;
    dct:hasPart C2004A01224:103,
        C2004A01224:104,
        C2004A01224:105,
        C2004A01224:106,
        C2004A01224:107,
        C2004A01224:108,
        C2004A01224:109,
        C2004A01224:110,
        C2004A01224:111,
        C2004A01224:112,
        C2004A01224:113 ;
    rdfs:comment "Chapter 4 Miscellaneous - Abrievated Graph Key: C102"@en-AU ;
    rdfs:subClassOf C2004A01224: ;
    skos:broader C2004A01224:103,
        C2004A01224:104,
        C2004A01224:105,
        C2004A01224:106,
        C2004A01224:107,
        C2004A01224:108,
        C2004A01224:109,
        C2004A01224:110,
        C2004A01224:111,
        C2004A01224:112,
        C2004A01224:113 ;
    skos:definition "Chapter 4 Miscellaneous"@en-AU ;
    skos:prefLabel "Chapter C102"@en-AU ;
    dcat:accessURL <https://www.legislation.gov.au/C2004A01224/2019-02-24/2019-02-24/text/1/epub/OEBPS/document_1/document_1.html#_Toc1469222> ;
    dcat:landingPage "https://www.legislation.gov.au/C2004A01224/2019-02-24/2019-02-24/text/1/epub/OEBPS/document_1/document_1.html#_Toc1469222"^^xsd:anyURI ;
    dcat:theme legcons:Chapter .

C2004A01224:60 a legcons:Chapter,
        C2004A01224:Chapter,
        owl:Class,
        dcat:Resource ;
    rdfs:label "Chapter - C60 Chapter 3 Legislative instruments and notifiable instruments"@en-AU ;
    dct:hasPart C2004A01224:100,
        C2004A01224:101,
        C2004A01224:61,
        C2004A01224:66,
        C2004A01224:79,
        C2004A01224:93,
        C2004A01224:94,
        C2004A01224:95,
        C2004A01224:96,
        C2004A01224:97,
        C2004A01224:98,
        C2004A01224:99 ;
    rdfs:comment "Chapter 3 Legislative instruments and notifiable instruments - Abrievated Graph Key: C60"@en-AU ;
    rdfs:subClassOf C2004A01224: ;
    skos:broader C2004A01224:100,
        C2004A01224:101,
        C2004A01224:61,
        C2004A01224:66,
        C2004A01224:79,
        C2004A01224:93,
        C2004A01224:94,
        C2004A01224:95,
        C2004A01224:96,
        C2004A01224:97,
        C2004A01224:98,
        C2004A01224:99 ;
    skos:definition "Chapter 3 Legislative instruments and notifiable instruments"@en-AU ;
    skos:prefLabel "Chapter C60"@en-AU ;
    dcat:accessURL <https://www.legislation.gov.au/C2004A01224/2019-02-24/2019-02-24/text/1/epub/OEBPS/document_1/document_1.html#_Toc1469180> ;
    dcat:landingPage "https://www.legislation.gov.au/C2004A01224/2019-02-24/2019-02-24/text/1/epub/OEBPS/document_1/document_1.html#_Toc1469180"^^xsd:anyURI ;
    dcat:theme legcons:Chapter .

C2004A01224:66 a legcons:Part,
        C2004A01224:Part,
        owl:Class,
        dcat:Resource ;
    rdfs:label "Part - P66 Part 2 Parliamentary scrutiny of legislative instruments"@en-AU ;
    dct:hasPart C2004A01224:67,
        C2004A01224:68,
        C2004A01224:69,
        C2004A01224:70,
        C2004A01224:71,
        C2004A01224:72,
        C2004A01224:73,
        C2004A01224:74,
        C2004A01224:75,
        C2004A01224:76,
        C2004A01224:77,
        C2004A01224:78 ;
    dct:isPartOf C2004A01224:60 ;
    rdfs:comment "Part 2 Parliamentary scrutiny of legislative instruments - Abrievated Graph Key: P66"@en-AU ;
    rdfs:subClassOf C2004A01224: ;
    skos:broader C2004A01224:67,
        C2004A01224:68,
        C2004A01224:69,
        C2004A01224:70,
        C2004A01224:71,
        C2004A01224:72,
        C2004A01224:73,
        C2004A01224:74,
        C2004A01224:75,
        C2004A01224:76,
        C2004A01224:77,
        C2004A01224:78 ;
    skos:definition "Part 2 Parliamentary scrutiny of legislative instruments"@en-AU ;
    skos:narrower C2004A01224:60 ;
    skos:prefLabel "Part P66"@en-AU ;
    dcat:accessURL <https://www.legislation.gov.au/C2004A01224/2019-02-24/2019-02-24/text/1/epub/OEBPS/document_1/document_1.html#_Toc1469186> ;
    dcat:landingPage "https://www.legislation.gov.au/C2004A01224/2019-02-24/2019-02-24/text/1/epub/OEBPS/document_1/document_1.html#_Toc1469186"^^xsd:anyURI ;
    dcat:theme legcons:Part .

C2004A01224:21 a legcons:Part,
        C2004A01224:Part,
        owl:Class,
        dcat:Resource ;
    rdfs:label "Part - P21 Part 1 The Federal Register of Legislation"@en-AU ;
    dct:hasPart C2004A01224:22,
        C2004A01224:24,
        C2004A01224:25,
        C2004A01224:26,
        C2004A01224:27,
        C2004A01224:28,
        C2004A01224:29,
        C2004A01224:30,
        C2004A01224:31,
        C2004A01224:32,
        C2004A01224:33,
        C2004A01224:34,
        C2004A01224:35,
        C2004A01224:36,
        C2004A01224:37,
        C2004A01224:38 ;
    dct:isPartOf C2004A01224:20 ;
    rdfs:comment "Part 1 The Federal Register of Legislation - Abrievated Graph Key: P21"@en-AU ;
    rdfs:subClassOf C2004A01224: ;
    skos:broader C2004A01224:22,
        C2004A01224:24,
        C2004A01224:25,
        C2004A01224:26,
        C2004A01224:27,
        C2004A01224:28,
        C2004A01224:29,
        C2004A01224:30,
        C2004A01224:31,
        C2004A01224:32,
        C2004A01224:33,
        C2004A01224:34,
        C2004A01224:35,
        C2004A01224:36,
        C2004A01224:37,
        C2004A01224:38 ;
    skos:definition "Part 1 The Federal Register of Legislation"@en-AU ;
    skos:narrower C2004A01224:20 ;
    skos:prefLabel "Part P21"@en-AU ;
    dcat:accessURL <https://www.legislation.gov.au/C2004A01224/2019-02-24/2019-02-24/text/1/epub/OEBPS/document_1/document_1.html#_Toc1469141> ;
    dcat:landingPage "https://www.legislation.gov.au/C2004A01224/2019-02-24/2019-02-24/text/1/epub/OEBPS/document_1/document_1.html#_Toc1469141"^^xsd:anyURI ;
    dcat:theme legcons:Part .

C2004A01224:1 a legcons:Chapter,
        C2004A01224:Chapter,
        owl:Class,
        dcat:Resource ;
    rdfs:label "Chapter - C1 Chapter 1 Introduction"@en-AU ;
    dct:hasPart C2004A01224:10,
        C2004A01224:11,
        C2004A01224:12,
        C2004A01224:13,
        C2004A01224:14,
        C2004A01224:15,
        C2004A01224:16,
        C2004A01224:17,
        C2004A01224:18,
        C2004A01224:19,
        C2004A01224:2,
        C2004A01224:3,
        C2004A01224:4,
        C2004A01224:5,
        C2004A01224:6,
        C2004A01224:7,
        C2004A01224:8,
        C2004A01224:9 ;
    rdfs:comment "Chapter 1 Introduction - Abrievated Graph Key: C1"@en-AU ;
    rdfs:subClassOf C2004A01224: ;
    skos:broader C2004A01224:10,
        C2004A01224:11,
        C2004A01224:12,
        C2004A01224:13,
        C2004A01224:14,
        C2004A01224:15,
        C2004A01224:16,
        C2004A01224:17,
        C2004A01224:18,
        C2004A01224:19,
        C2004A01224:2,
        C2004A01224:3,
        C2004A01224:4,
        C2004A01224:5,
        C2004A01224:6,
        C2004A01224:7,
        C2004A01224:8,
        C2004A01224:9 ;
    skos:definition "Chapter 1 Introduction"@en-AU ;
    skos:prefLabel "Chapter C1"@en-AU ;
    dcat:accessURL <https://www.legislation.gov.au/C2004A01224/2019-02-24/2019-02-24/text/1/epub/OEBPS/document_1/document_1.html#_Toc1469121> ;
    dcat:landingPage "https://www.legislation.gov.au/C2004A01224/2019-02-24/2019-02-24/text/1/epub/OEBPS/document_1/document_1.html#_Toc1469121"^^xsd:anyURI ;
    dcat:theme legcons:Chapter .

C2004A01224: a owl:Class,
        dcat:Dataset,
        dcat:Resource ;
    rdfs:label "Legislation Act 2003" ;
    dct:Jurisdiction " Attorney-General's Department "@en-AU ;
    dct:created "2024-08-22T23:18:30.324505"^^xsd:dateTime ;
    dct:creator "https://orcid.org/0009-0007-8434-7325"^^xsd:anyURI ;
    dct:date "2019-02-24T00:00:00+11:00"^^xsd:dateTime ;
    dct:description "Legislation Act 2003"@en-AU ;
    dct:identifier "https://www.legislation.gov.au/C2004A01224/latest"^^xsd:anyURI ;
    dct:license <https://creativecommons.org/licenses/by-sa/4.0/> ;
    dct:source "scheme=AGLSTERMS.AglsAgent; corporateName=Office Parliamentary Counsel; address=Locked Bag 30 Kingston ACT 2604; contact=+61 2 6120 1400"@en-AU ;
    dct:subject "Legislation Act 2003"@en-AU ;
    dct:title "Legislation Act 2003"@en-AU ;
    owl:imports legcons: ;
    dcat:theme legcons:Chapter,
        legcons:Division,
        legcons:Endnotes,
        legcons:Item,
        legcons:Part,
        legcons:Subdivision ;
    schema:identifier "C2004A01224" ;
    schema:status "In force" ;
    schema:version "C2019C00084 (C39)" .

