@prefix C2022A00037: <http://example.org/au/leg/dataset/C2022A00037/> .
@prefix dcat: <http://www.w3.org/ns/dcat#> .
@prefix dct: <http://purl.org/dc/terms/> .
@prefix legcons: <http://example.org/au/leg/concepts/> .
@prefix owl: <http://www.w3.org/2002/07/owl#> .
@prefix rdfs: <http://www.w3.org/2000/01/rdf-schema#> .
@prefix schema: <https://schema.org/> .
@prefix skos: <http://www.w3.org/2004/02/skos/core#> .
@prefix xsd: <http://www.w3.org/2001/XMLSchema#> .

C2022A00037:11 a legcons:Item,
        owl:Class,
        dcat:Resource ;
    rdfs:label "Item - I11 9  Simplified outline of this Part"@en-AU ;
    dct:isPartOf C2022A00037:10 ;
    rdfs:comment "9  Simplified outline of this Part - Abrievated Graph Key: I11"@en-AU ;
    rdfs:subClassOf C2022A00037: ;
    skos:definition "9  Simplified outline of this Part"@en-AU ;
    skos:narrower C2022A00037:10 ;
    skos:prefLabel "Item I11"@en-AU ;
    dcat:accessURL <https://www.legislation.gov.au/C2022A00037/2023-04-12/2023-04-12/text/original/epub/OEBPS/document_1/document_1.html#_Toc133933914> ;
    dcat:landingPage "https://www.legislation.gov.au/C2022A00037/2023-04-12/2023-04-12/text/original/epub/OEBPS/document_1/document_1.html#_Toc133933914"^^xsd:anyURI .

C2022A00037:12 a legcons:Item,
        owl:Class,
        dcat:Resource ;
    rdfs:label "Item - I12 10  Australias greenhouse gas emissions reduction targets"@en-AU ;
    dct:isPartOf C2022A00037:10 ;
    rdfs:comment "10  Australias greenhouse gas emissions reduction targets - Abrievated Graph Key: I12"@en-AU ;
    rdfs:subClassOf C2022A00037: ;
    skos:definition "10  Australias greenhouse gas emissions reduction targets"@en-AU ;
    skos:narrower C2022A00037:10 ;
    skos:prefLabel "Item I12"@en-AU ;
    dcat:accessURL <https://www.legislation.gov.au/C2022A00037/2023-04-12/2023-04-12/text/original/epub/OEBPS/document_1/document_1.html#_Toc133933915> ;
    dcat:landingPage "https://www.legislation.gov.au/C2022A00037/2023-04-12/2023-04-12/text/original/epub/OEBPS/document_1/document_1.html#_Toc133933915"^^xsd:anyURI .

C2022A00037:14 a legcons:Item,
        owl:Class,
        dcat:Resource ;
    rdfs:label "Item - I14 11  Simplified outline of this Part"@en-AU ;
    dct:isPartOf C2022A00037:13 ;
    rdfs:comment "11  Simplified outline of this Part - Abrievated Graph Key: I14"@en-AU ;
    rdfs:subClassOf C2022A00037: ;
    skos:definition "11  Simplified outline of this Part"@en-AU ;
    skos:narrower C2022A00037:13 ;
    skos:prefLabel "Item I14"@en-AU ;
    dcat:accessURL <https://www.legislation.gov.au/C2022A00037/2023-04-12/2023-04-12/text/original/epub/OEBPS/document_1/document_1.html#_Toc133933917> ;
    dcat:landingPage "https://www.legislation.gov.au/C2022A00037/2023-04-12/2023-04-12/text/original/epub/OEBPS/document_1/document_1.html#_Toc133933917"^^xsd:anyURI .

C2022A00037:15 a legcons:Item,
        owl:Class,
        dcat:Resource ;
    rdfs:label "Item - I15 12  Annual climate change statement"@en-AU ;
    dct:isPartOf C2022A00037:13 ;
    rdfs:comment "12  Annual climate change statement - Abrievated Graph Key: I15"@en-AU ;
    rdfs:subClassOf C2022A00037: ;
    skos:definition "12  Annual climate change statement"@en-AU ;
    skos:narrower C2022A00037:13 ;
    skos:prefLabel "Item I15"@en-AU ;
    dcat:accessURL <https://www.legislation.gov.au/C2022A00037/2023-04-12/2023-04-12/text/original/epub/OEBPS/document_1/document_1.html#_Toc133933918> ;
    dcat:landingPage "https://www.legislation.gov.au/C2022A00037/2023-04-12/2023-04-12/text/original/epub/OEBPS/document_1/document_1.html#_Toc133933918"^^xsd:anyURI .

C2022A00037:17 a legcons:Item,
        owl:Class,
        dcat:Resource ;
    rdfs:label "Item - I17 13  Simplified outline of this Part"@en-AU ;
    dct:isPartOf C2022A00037:16 ;
    rdfs:comment "13  Simplified outline of this Part - Abrievated Graph Key: I17"@en-AU ;
    rdfs:subClassOf C2022A00037: ;
    skos:definition "13  Simplified outline of this Part"@en-AU ;
    skos:narrower C2022A00037:16 ;
    skos:prefLabel "Item I17"@en-AU ;
    dcat:accessURL <https://www.legislation.gov.au/C2022A00037/2023-04-12/2023-04-12/text/original/epub/OEBPS/document_1/document_1.html#_Toc133933920> ;
    dcat:landingPage "https://www.legislation.gov.au/C2022A00037/2023-04-12/2023-04-12/text/original/epub/OEBPS/document_1/document_1.html#_Toc133933920"^^xsd:anyURI .

C2022A00037:18 a legcons:Item,
        owl:Class,
        dcat:Resource ;
    rdfs:label "Item - I18 14  Climate Change Authority to give the Minister advice that relates to the preparation of an annual climate change statement"@en-AU ;
    dct:isPartOf C2022A00037:16 ;
    rdfs:comment "14  Climate Change Authority to give the Minister advice that relates to the preparation of an annual climate change statement - Abrievated Graph Key: I18"@en-AU ;
    rdfs:subClassOf C2022A00037: ;
    skos:definition "14  Climate Change Authority to give the Minister advice that relates to the preparation of an annual climate change statement"@en-AU ;
    skos:narrower C2022A00037:16 ;
    skos:prefLabel "Item I18"@en-AU ;
    dcat:accessURL <https://www.legislation.gov.au/C2022A00037/2023-04-12/2023-04-12/text/original/epub/OEBPS/document_1/document_1.html#_Toc133933921> ;
    dcat:landingPage "https://www.legislation.gov.au/C2022A00037/2023-04-12/2023-04-12/text/original/epub/OEBPS/document_1/document_1.html#_Toc133933921"^^xsd:anyURI .

C2022A00037:19 a legcons:Item,
        owl:Class,
        dcat:Resource ;
    rdfs:label "Item - I19 15  Climate Change Authority to advise the Minister on greenhouse gas emissions reduction targets to be included in a new or adjusted nationally determined contribution"@en-AU ;
    dct:isPartOf C2022A00037:16 ;
    rdfs:comment "15  Climate Change Authority to advise the Minister on greenhouse gas emissions reduction targets to be included in a new or adjusted nationally determined contribution - Abrievated Graph Key: I19"@en-AU ;
    rdfs:subClassOf C2022A00037: ;
    skos:definition "15  Climate Change Authority to advise the Minister on greenhouse gas emissions reduction targets to be included in a new or adjusted nationally determined contribution"@en-AU ;
    skos:narrower C2022A00037:16 ;
    skos:prefLabel "Item I19"@en-AU ;
    dcat:accessURL <https://www.legislation.gov.au/C2022A00037/2023-04-12/2023-04-12/text/original/epub/OEBPS/document_1/document_1.html#_Toc133933922> ;
    dcat:landingPage "https://www.legislation.gov.au/C2022A00037/2023-04-12/2023-04-12/text/original/epub/OEBPS/document_1/document_1.html#_Toc133933922"^^xsd:anyURI .

C2022A00037:2 a legcons:Item,
        owl:Class,
        dcat:Resource ;
    rdfs:label "Item - I2 1  Short title"@en-AU ;
    dct:isPartOf C2022A00037:1 ;
    rdfs:comment "1  Short title - Abrievated Graph Key: I2"@en-AU ;
    rdfs:subClassOf C2022A00037: ;
    skos:definition "1  Short title"@en-AU ;
    skos:narrower C2022A00037:1 ;
    skos:prefLabel "Item I2"@en-AU ;
    dcat:accessURL <https://www.legislation.gov.au/C2022A00037/2023-04-12/2023-04-12/text/original/epub/OEBPS/document_1/document_1.html#_Toc133933905> ;
    dcat:landingPage "https://www.legislation.gov.au/C2022A00037/2023-04-12/2023-04-12/text/original/epub/OEBPS/document_1/document_1.html#_Toc133933905"^^xsd:anyURI .

C2022A00037:20 a legcons:Item,
        owl:Class,
        dcat:Resource ;
    rdfs:label "Item - I20 15 A  Environment Minister to give Minister Climate Change Secretary and Climate Change Authority certain emissions estimates"@en-AU ;
    dct:isPartOf C2022A00037:16 ;
    rdfs:comment "15 A  Environment Minister to give Minister Climate Change Secretary and Climate Change Authority certain emissions estimates - Abrievated Graph Key: I20"@en-AU ;
    rdfs:subClassOf C2022A00037: ;
    skos:definition "15 A  Environment Minister to give Minister Climate Change Secretary and Climate Change Authority certain emissions estimates"@en-AU ;
    skos:narrower C2022A00037:16 ;
    skos:prefLabel "Item I20"@en-AU ;
    dcat:accessURL <https://www.legislation.gov.au/C2022A00037/2023-04-12/2023-04-12/text/original/epub/OEBPS/document_1/document_1.html#_Toc133933923> ;
    dcat:landingPage "https://www.legislation.gov.au/C2022A00037/2023-04-12/2023-04-12/text/original/epub/OEBPS/document_1/document_1.html#_Toc133933923"^^xsd:anyURI .

C2022A00037:22 a legcons:Item,
        owl:Class,
        dcat:Resource ;
    rdfs:label "Item - I22 16  Simplified outline of this Part"@en-AU ;
    dct:isPartOf C2022A00037:21 ;
    rdfs:comment "16  Simplified outline of this Part - Abrievated Graph Key: I22"@en-AU ;
    rdfs:subClassOf C2022A00037: ;
    skos:definition "16  Simplified outline of this Part"@en-AU ;
    skos:narrower C2022A00037:21 ;
    skos:prefLabel "Item I22"@en-AU ;
    dcat:accessURL <https://www.legislation.gov.au/C2022A00037/2023-04-12/2023-04-12/text/original/epub/OEBPS/document_1/document_1.html#_Toc133933925> ;
    dcat:landingPage "https://www.legislation.gov.au/C2022A00037/2023-04-12/2023-04-12/text/original/epub/OEBPS/document_1/document_1.html#_Toc133933925"^^xsd:anyURI .

C2022A00037:23 a legcons:Item,
        owl:Class,
        dcat:Resource ;
    rdfs:label "Item - I23 17  Periodic reviews of the operation of this Act"@en-AU ;
    dct:isPartOf C2022A00037:21 ;
    rdfs:comment "17  Periodic reviews of the operation of this Act - Abrievated Graph Key: I23"@en-AU ;
    rdfs:subClassOf C2022A00037: ;
    skos:definition "17  Periodic reviews of the operation of this Act"@en-AU ;
    skos:narrower C2022A00037:21 ;
    skos:prefLabel "Item I23"@en-AU ;
    dcat:accessURL <https://www.legislation.gov.au/C2022A00037/2023-04-12/2023-04-12/text/original/epub/OEBPS/document_1/document_1.html#_Toc133933926> ;
    dcat:landingPage "https://www.legislation.gov.au/C2022A00037/2023-04-12/2023-04-12/text/original/epub/OEBPS/document_1/document_1.html#_Toc133933926"^^xsd:anyURI .

C2022A00037:25 a legcons:Item,
        owl:Class,
        dcat:Resource ;
    rdfs:label "Item - I25 Endnote 1 About the endnotes"@en-AU ;
    dct:isPartOf C2022A00037:24 ;
    rdfs:comment "Endnote 1 About the endnotes - Abrievated Graph Key: I25"@en-AU ;
    rdfs:subClassOf C2022A00037: ;
    skos:definition "Endnote 1 About the endnotes"@en-AU ;
    skos:narrower C2022A00037:24 ;
    skos:prefLabel "Item I25"@en-AU ;
    dcat:accessURL <https://www.legislation.gov.au/C2022A00037/2023-04-12/2023-04-12/text/original/epub/OEBPS/document_1/document_1.html#_Toc133933928> ;
    dcat:landingPage "https://www.legislation.gov.au/C2022A00037/2023-04-12/2023-04-12/text/original/epub/OEBPS/document_1/document_1.html#_Toc133933928"^^xsd:anyURI .

C2022A00037:26 a legcons:Item,
        owl:Class,
        dcat:Resource ;
    rdfs:label "Item - I26 Endnote 2 Abbreviation key"@en-AU ;
    dct:isPartOf C2022A00037:24 ;
    rdfs:comment "Endnote 2 Abbreviation key - Abrievated Graph Key: I26"@en-AU ;
    rdfs:subClassOf C2022A00037: ;
    skos:definition "Endnote 2 Abbreviation key"@en-AU ;
    skos:narrower C2022A00037:24 ;
    skos:prefLabel "Item I26"@en-AU ;
    dcat:accessURL <https://www.legislation.gov.au/C2022A00037/2023-04-12/2023-04-12/text/original/epub/OEBPS/document_1/document_1.html#_Toc133933929> ;
    dcat:landingPage "https://www.legislation.gov.au/C2022A00037/2023-04-12/2023-04-12/text/original/epub/OEBPS/document_1/document_1.html#_Toc133933929"^^xsd:anyURI .

C2022A00037:27 a legcons:Item,
        owl:Class,
        dcat:Resource ;
    rdfs:label "Item - I27 Endnote 3 Legislation history"@en-AU ;
    dct:isPartOf C2022A00037:24 ;
    rdfs:comment "Endnote 3 Legislation history - Abrievated Graph Key: I27"@en-AU ;
    rdfs:subClassOf C2022A00037: ;
    skos:definition "Endnote 3 Legislation history"@en-AU ;
    skos:narrower C2022A00037:24 ;
    skos:prefLabel "Item I27"@en-AU ;
    dcat:accessURL <https://www.legislation.gov.au/C2022A00037/2023-04-12/2023-04-12/text/original/epub/OEBPS/document_1/document_1.html#_Toc133933930> ;
    dcat:landingPage "https://www.legislation.gov.au/C2022A00037/2023-04-12/2023-04-12/text/original/epub/OEBPS/document_1/document_1.html#_Toc133933930"^^xsd:anyURI .

C2022A00037:28 a legcons:Item,
        owl:Class,
        dcat:Resource ;
    rdfs:label "Item - I28 Endnote 4 Amendment history"@en-AU ;
    dct:isPartOf C2022A00037:24 ;
    rdfs:comment "Endnote 4 Amendment history - Abrievated Graph Key: I28"@en-AU ;
    rdfs:subClassOf C2022A00037: ;
    skos:definition "Endnote 4 Amendment history"@en-AU ;
    skos:narrower C2022A00037:24 ;
    skos:prefLabel "Item I28"@en-AU ;
    dcat:accessURL <https://www.legislation.gov.au/C2022A00037/2023-04-12/2023-04-12/text/original/epub/OEBPS/document_1/document_1.html#_Toc133933931> ;
    dcat:landingPage "https://www.legislation.gov.au/C2022A00037/2023-04-12/2023-04-12/text/original/epub/OEBPS/document_1/document_1.html#_Toc133933931"^^xsd:anyURI .

C2022A00037:3 a legcons:Item,
        owl:Class,
        dcat:Resource ;
    rdfs:label "Item - I3 2  Commencement"@en-AU ;
    dct:isPartOf C2022A00037:1 ;
    rdfs:comment "2  Commencement - Abrievated Graph Key: I3"@en-AU ;
    rdfs:subClassOf C2022A00037: ;
    skos:definition "2  Commencement"@en-AU ;
    skos:narrower C2022A00037:1 ;
    skos:prefLabel "Item I3"@en-AU ;
    dcat:accessURL <https://www.legislation.gov.au/C2022A00037/2023-04-12/2023-04-12/text/original/epub/OEBPS/document_1/document_1.html#_Toc133933906> ;
    dcat:landingPage "https://www.legislation.gov.au/C2022A00037/2023-04-12/2023-04-12/text/original/epub/OEBPS/document_1/document_1.html#_Toc133933906"^^xsd:anyURI .

C2022A00037:4 a legcons:Item,
        owl:Class,
        dcat:Resource ;
    rdfs:label "Item - I4 3  Objects"@en-AU ;
    dct:isPartOf C2022A00037:1 ;
    rdfs:comment "3  Objects - Abrievated Graph Key: I4"@en-AU ;
    rdfs:subClassOf C2022A00037: ;
    skos:definition "3  Objects"@en-AU ;
    skos:narrower C2022A00037:1 ;
    skos:prefLabel "Item I4"@en-AU ;
    dcat:accessURL <https://www.legislation.gov.au/C2022A00037/2023-04-12/2023-04-12/text/original/epub/OEBPS/document_1/document_1.html#_Toc133933907> ;
    dcat:landingPage "https://www.legislation.gov.au/C2022A00037/2023-04-12/2023-04-12/text/original/epub/OEBPS/document_1/document_1.html#_Toc133933907"^^xsd:anyURI .

C2022A00037:5 a legcons:Item,
        owl:Class,
        dcat:Resource ;
    rdfs:label "Item - I5 4  Simplified outline of this Act"@en-AU ;
    dct:isPartOf C2022A00037:1 ;
    rdfs:comment "4  Simplified outline of this Act - Abrievated Graph Key: I5"@en-AU ;
    rdfs:subClassOf C2022A00037: ;
    skos:definition "4  Simplified outline of this Act"@en-AU ;
    skos:narrower C2022A00037:1 ;
    skos:prefLabel "Item I5"@en-AU ;
    dcat:accessURL <https://www.legislation.gov.au/C2022A00037/2023-04-12/2023-04-12/text/original/epub/OEBPS/document_1/document_1.html#_Toc133933908> ;
    dcat:landingPage "https://www.legislation.gov.au/C2022A00037/2023-04-12/2023-04-12/text/original/epub/OEBPS/document_1/document_1.html#_Toc133933908"^^xsd:anyURI .

C2022A00037:6 a legcons:Item,
        owl:Class,
        dcat:Resource ;
    rdfs:label "Item - I6 5  Definitions"@en-AU ;
    dct:isPartOf C2022A00037:1 ;
    rdfs:comment "5  Definitions - Abrievated Graph Key: I6"@en-AU ;
    rdfs:subClassOf C2022A00037: ;
    skos:definition "5  Definitions"@en-AU ;
    skos:narrower C2022A00037:1 ;
    skos:prefLabel "Item I6"@en-AU ;
    dcat:accessURL <https://www.legislation.gov.au/C2022A00037/2023-04-12/2023-04-12/text/original/epub/OEBPS/document_1/document_1.html#_Toc133933909> ;
    dcat:landingPage "https://www.legislation.gov.au/C2022A00037/2023-04-12/2023-04-12/text/original/epub/OEBPS/document_1/document_1.html#_Toc133933909"^^xsd:anyURI .

C2022A00037:7 a legcons:Item,
        owl:Class,
        dcat:Resource ;
    rdfs:label "Item - I7 6  Act binds the Crown"@en-AU ;
    dct:isPartOf C2022A00037:1 ;
    rdfs:comment "6  Act binds the Crown - Abrievated Graph Key: I7"@en-AU ;
    rdfs:subClassOf C2022A00037: ;
    skos:definition "6  Act binds the Crown"@en-AU ;
    skos:narrower C2022A00037:1 ;
    skos:prefLabel "Item I7"@en-AU ;
    dcat:accessURL <https://www.legislation.gov.au/C2022A00037/2023-04-12/2023-04-12/text/original/epub/OEBPS/document_1/document_1.html#_Toc133933910> ;
    dcat:landingPage "https://www.legislation.gov.au/C2022A00037/2023-04-12/2023-04-12/text/original/epub/OEBPS/document_1/document_1.html#_Toc133933910"^^xsd:anyURI .

C2022A00037:8 a legcons:Item,
        owl:Class,
        dcat:Resource ;
    rdfs:label "Item - I8 7  Extension to external Territories"@en-AU ;
    dct:isPartOf C2022A00037:1 ;
    rdfs:comment "7  Extension to external Territories - Abrievated Graph Key: I8"@en-AU ;
    rdfs:subClassOf C2022A00037: ;
    skos:definition "7  Extension to external Territories"@en-AU ;
    skos:narrower C2022A00037:1 ;
    skos:prefLabel "Item I8"@en-AU ;
    dcat:accessURL <https://www.legislation.gov.au/C2022A00037/2023-04-12/2023-04-12/text/original/epub/OEBPS/document_1/document_1.html#_Toc133933911> ;
    dcat:landingPage "https://www.legislation.gov.au/C2022A00037/2023-04-12/2023-04-12/text/original/epub/OEBPS/document_1/document_1.html#_Toc133933911"^^xsd:anyURI .

C2022A00037:9 a legcons:Item,
        owl:Class,
        dcat:Resource ;
    rdfs:label "Item - I9 8  Extension to exclusive economic zone and continental shelf"@en-AU ;
    dct:isPartOf C2022A00037:1 ;
    rdfs:comment "8  Extension to exclusive economic zone and continental shelf - Abrievated Graph Key: I9"@en-AU ;
    rdfs:subClassOf C2022A00037: ;
    skos:definition "8  Extension to exclusive economic zone and continental shelf"@en-AU ;
    skos:narrower C2022A00037:1 ;
    skos:prefLabel "Item I9"@en-AU ;
    dcat:accessURL <https://www.legislation.gov.au/C2022A00037/2023-04-12/2023-04-12/text/original/epub/OEBPS/document_1/document_1.html#_Toc133933912> ;
    dcat:landingPage "https://www.legislation.gov.au/C2022A00037/2023-04-12/2023-04-12/text/original/epub/OEBPS/document_1/document_1.html#_Toc133933912"^^xsd:anyURI .

C2022A00037:10 a legcons:Part,
        owl:Class,
        dcat:Resource ;
    rdfs:label "Part - P10 Part 2 Australias greenhouse gas emissions reduction targets"@en-AU ;
    dct:hasPart C2022A00037:11,
        C2022A00037:12 ;
    rdfs:comment "Part 2 Australias greenhouse gas emissions reduction targets - Abrievated Graph Key: P10"@en-AU ;
    rdfs:subClassOf C2022A00037: ;
    skos:broader C2022A00037:11,
        C2022A00037:12 ;
    skos:definition "Part 2 Australias greenhouse gas emissions reduction targets"@en-AU ;
    skos:prefLabel "Part P10"@en-AU ;
    dcat:accessURL <https://www.legislation.gov.au/C2022A00037/2023-04-12/2023-04-12/text/original/epub/OEBPS/document_1/document_1.html#_Toc133933913> ;
    dcat:landingPage "https://www.legislation.gov.au/C2022A00037/2023-04-12/2023-04-12/text/original/epub/OEBPS/document_1/document_1.html#_Toc133933913"^^xsd:anyURI .

C2022A00037:13 a legcons:Part,
        owl:Class,
        dcat:Resource ;
    rdfs:label "Part - P13 Part 3 Annual climate change statement"@en-AU ;
    dct:hasPart C2022A00037:14,
        C2022A00037:15 ;
    rdfs:comment "Part 3 Annual climate change statement - Abrievated Graph Key: P13"@en-AU ;
    rdfs:subClassOf C2022A00037: ;
    skos:broader C2022A00037:14,
        C2022A00037:15 ;
    skos:definition "Part 3 Annual climate change statement"@en-AU ;
    skos:prefLabel "Part P13"@en-AU ;
    dcat:accessURL <https://www.legislation.gov.au/C2022A00037/2023-04-12/2023-04-12/text/original/epub/OEBPS/document_1/document_1.html#_Toc133933916> ;
    dcat:landingPage "https://www.legislation.gov.au/C2022A00037/2023-04-12/2023-04-12/text/original/epub/OEBPS/document_1/document_1.html#_Toc133933916"^^xsd:anyURI .

C2022A00037:21 a legcons:Part,
        owl:Class,
        dcat:Resource ;
    rdfs:label "Part - P21 Part 5 Periodic reviews of the operation of this Act"@en-AU ;
    dct:hasPart C2022A00037:22,
        C2022A00037:23 ;
    rdfs:comment "Part 5 Periodic reviews of the operation of this Act - Abrievated Graph Key: P21"@en-AU ;
    rdfs:subClassOf C2022A00037: ;
    skos:broader C2022A00037:22,
        C2022A00037:23 ;
    skos:definition "Part 5 Periodic reviews of the operation of this Act"@en-AU ;
    skos:prefLabel "Part P21"@en-AU ;
    dcat:accessURL <https://www.legislation.gov.au/C2022A00037/2023-04-12/2023-04-12/text/original/epub/OEBPS/document_1/document_1.html#_Toc133933924> ;
    dcat:landingPage "https://www.legislation.gov.au/C2022A00037/2023-04-12/2023-04-12/text/original/epub/OEBPS/document_1/document_1.html#_Toc133933924"^^xsd:anyURI .

C2022A00037:16 a legcons:Part,
        owl:Class,
        dcat:Resource ;
    rdfs:label "Part - P16 Part 4 Advisory functions of the Climate Change Authority etc"@en-AU ;
    dct:hasPart C2022A00037:17,
        C2022A00037:18,
        C2022A00037:19,
        C2022A00037:20 ;
    rdfs:comment "Part 4 Advisory functions of the Climate Change Authority etc - Abrievated Graph Key: P16"@en-AU ;
    rdfs:subClassOf C2022A00037: ;
    skos:broader C2022A00037:17,
        C2022A00037:18,
        C2022A00037:19,
        C2022A00037:20 ;
    skos:definition "Part 4 Advisory functions of the Climate Change Authority etc"@en-AU ;
    skos:prefLabel "Part P16"@en-AU ;
    dcat:accessURL <https://www.legislation.gov.au/C2022A00037/2023-04-12/2023-04-12/text/original/epub/OEBPS/document_1/document_1.html#_Toc133933919> ;
    dcat:landingPage "https://www.legislation.gov.au/C2022A00037/2023-04-12/2023-04-12/text/original/epub/OEBPS/document_1/document_1.html#_Toc133933919"^^xsd:anyURI .

C2022A00037:24 a legcons:Endnotes,
        owl:Class,
        dcat:Resource ;
    rdfs:label "Endnotes - E24 Endnotes"@en-AU ;
    dct:hasPart C2022A00037:25,
        C2022A00037:26,
        C2022A00037:27,
        C2022A00037:28 ;
    rdfs:comment "Endnotes - Abrievated Graph Key: E24"@en-AU ;
    rdfs:subClassOf C2022A00037: ;
    skos:broader C2022A00037:25,
        C2022A00037:26,
        C2022A00037:27,
        C2022A00037:28 ;
    skos:definition "Endnotes"@en-AU ;
    skos:prefLabel "Endnotes E24"@en-AU ;
    dcat:accessURL <https://www.legislation.gov.au/C2022A00037/2023-04-12/2023-04-12/text/original/epub/OEBPS/document_1/document_1.html#_Toc133933927> ;
    dcat:landingPage "https://www.legislation.gov.au/C2022A00037/2023-04-12/2023-04-12/text/original/epub/OEBPS/document_1/document_1.html#_Toc133933927"^^xsd:anyURI .

C2022A00037:1 a legcons:Part,
        owl:Class,
        dcat:Resource ;
    rdfs:label "Part - P1 Part 1 Preliminary"@en-AU ;
    dct:hasPart C2022A00037:2,
        C2022A00037:3,
        C2022A00037:4,
        C2022A00037:5,
        C2022A00037:6,
        C2022A00037:7,
        C2022A00037:8,
        C2022A00037:9 ;
    rdfs:comment "Part 1 Preliminary - Abrievated Graph Key: P1"@en-AU ;
    rdfs:subClassOf C2022A00037: ;
    skos:broader C2022A00037:2,
        C2022A00037:3,
        C2022A00037:4,
        C2022A00037:5,
        C2022A00037:6,
        C2022A00037:7,
        C2022A00037:8,
        C2022A00037:9 ;
    skos:definition "Part 1 Preliminary"@en-AU ;
    skos:prefLabel "Part P1"@en-AU ;
    dcat:accessURL <https://www.legislation.gov.au/C2022A00037/2023-04-12/2023-04-12/text/original/epub/OEBPS/document_1/document_1.html#_Toc133933904> ;
    dcat:landingPage "https://www.legislation.gov.au/C2022A00037/2023-04-12/2023-04-12/text/original/epub/OEBPS/document_1/document_1.html#_Toc133933904"^^xsd:anyURI .

C2022A00037: a owl:Class,
        dcat:Dataset,
        dcat:Resource ;
    rdfs:label "Climate Change Act 2022" ;
    dct:Agent "Climate Change, Energy, the Environment and Water"@en-AU ;
    dct:created "2024-08-20T16:37:10.553293"^^xsd:dateTime ;
    dct:creator "https://orcid.org/0009-0007-8434-7325"^^xsd:anyURI ;
    dct:date "2023-04-12T00:00:00+10:00"^^xsd:dateTime ;
    dct:description "Climate Change Act 2022"@en-AU ;
    dct:identifier "https://www.legislation.gov.au/C2022A00037/latest"^^xsd:anyURI ;
    dct:license <https://creativecommons.org/licenses/by-sa/4.0/> ;
    dct:publisher "Department of Climate Change, Energy, the Environment and Water" ;
    dct:source "scheme=AGLSTERMS.AglsAgent; corporateName=Office Parliamentary Counsel; address=Locked Bag 30 Kingston ACT 2604; contact=+61 2 6120 1400"@en-AU ;
    dct:subject "Climate Change Act 2022"@en-AU ;
    dct:title "Climate Change Act 2022"@en-AU ;
    dcat:theme legcons:Endnotes,
        legcons:Item,
        legcons:Part ;
    schema:identifier "C2022A00037" ;
    schema:status "In force" ;
    schema:version "C2023C00092 (C01)" .

