@prefix C2024A00059: <http://example.org/au/leg/dataset/C2024A00059/> .
@prefix dcat: <http://www.w3.org/ns/dcat#> .
@prefix dct: <http://purl.org/dc/terms/> .
@prefix legcons: <http://example.org/au/leg/concepts/> .
@prefix owl: <http://www.w3.org/2002/07/owl#> .
@prefix rdfs: <http://www.w3.org/2000/01/rdf-schema#> .
@prefix schema: <https://schema.org/> .
@prefix skos: <http://www.w3.org/2004/02/skos/core#> .
@prefix xsd: <http://www.w3.org/2001/XMLSchema#> .

C2024A00059:10 a legcons:Item,
        owl:Class,
        dcat:Resource ;
    rdfs:label "Item - I10 9  Definition of research and development activity"@en-AU ;
    dct:isPartOf C2024A00059:1 ;
    dct:isReferencedBy C2024A00059: ;
    rdfs:comment "9  Definition of research and development activity - Abrievated Graph Key: I10"@en-AU ;
    skos:definition "9  Definition of research and development activity"@en-AU ;
    skos:narrower C2024A00059:1 ;
    skos:prefLabel "Item I10"@en-AU ;
    dcat:accessURL <https://www.legislation.gov.au/C2024A00059/asmade/2024-07-09/text/original/epub/OEBPS/document_1/document_1.html#_Toc171508565> ;
    dcat:landingPage "https://www.legislation.gov.au/C2024A00059/asmade/2024-07-09/text/original/epub/OEBPS/document_1/document_1.html#_Toc171508565"^^xsd:anyURI ;
    dcat:theme legcons:Item .

C2024A00059:102 a legcons:Item,
        owl:Class,
        dcat:Resource ;
    rdfs:label "Item - I102 68  Use or disclosure for National Residue Survey activities etc"@en-AU ;
    dct:isPartOf C2024A00059:101 ;
    dct:isReferencedBy C2024A00059: ;
    rdfs:comment "68  Use or disclosure for National Residue Survey activities etc - Abrievated Graph Key: I102"@en-AU ;
    skos:definition "68  Use or disclosure for National Residue Survey activities etc"@en-AU ;
    skos:narrower C2024A00059:101 ;
    skos:prefLabel "Item I102"@en-AU ;
    dcat:accessURL <https://www.legislation.gov.au/C2024A00059/asmade/2024-07-09/text/original/epub/OEBPS/document_1/document_1.html#_Toc171508657> ;
    dcat:landingPage "https://www.legislation.gov.au/C2024A00059/asmade/2024-07-09/text/original/epub/OEBPS/document_1/document_1.html#_Toc171508657"^^xsd:anyURI ;
    dcat:theme legcons:Item .

C2024A00059:103 a legcons:Item,
        owl:Class,
        dcat:Resource ;
    rdfs:label "Item - I103 69  Use or disclosure for the purposes of other Acts"@en-AU ;
    dct:isPartOf C2024A00059:101 ;
    dct:isReferencedBy C2024A00059: ;
    rdfs:comment "69  Use or disclosure for the purposes of other Acts - Abrievated Graph Key: I103"@en-AU ;
    skos:definition "69  Use or disclosure for the purposes of other Acts"@en-AU ;
    skos:narrower C2024A00059:101 ;
    skos:prefLabel "Item I103"@en-AU ;
    dcat:accessURL <https://www.legislation.gov.au/C2024A00059/asmade/2024-07-09/text/original/epub/OEBPS/document_1/document_1.html#_Toc171508658> ;
    dcat:landingPage "https://www.legislation.gov.au/C2024A00059/asmade/2024-07-09/text/original/epub/OEBPS/document_1/document_1.html#_Toc171508658"^^xsd:anyURI ;
    dcat:theme legcons:Item .

C2024A00059:104 a legcons:Item,
        owl:Class,
        dcat:Resource ;
    rdfs:label "Item - I104 70  Disclosure to authorities of the Commonwealth a State or Territory"@en-AU ;
    dct:isPartOf C2024A00059:101 ;
    dct:isReferencedBy C2024A00059: ;
    rdfs:comment "70  Disclosure to authorities of the Commonwealth a State or Territory - Abrievated Graph Key: I104"@en-AU ;
    skos:definition "70  Disclosure to authorities of the Commonwealth a State or Territory"@en-AU ;
    skos:narrower C2024A00059:101 ;
    skos:prefLabel "Item I104"@en-AU ;
    dcat:accessURL <https://www.legislation.gov.au/C2024A00059/asmade/2024-07-09/text/original/epub/OEBPS/document_1/document_1.html#_Toc171508659> ;
    dcat:landingPage "https://www.legislation.gov.au/C2024A00059/asmade/2024-07-09/text/original/epub/OEBPS/document_1/document_1.html#_Toc171508659"^^xsd:anyURI ;
    dcat:theme legcons:Item .

C2024A00059:105 a legcons:Item,
        owl:Class,
        dcat:Resource ;
    rdfs:label "Item - I105 71  Disclosure to foreign governments etc for export trade and other purposes"@en-AU ;
    dct:isPartOf C2024A00059:101 ;
    dct:isReferencedBy C2024A00059: ;
    rdfs:comment "71  Disclosure to foreign governments etc for export trade and other purposes - Abrievated Graph Key: I105"@en-AU ;
    skos:definition "71  Disclosure to foreign governments etc for export trade and other purposes"@en-AU ;
    skos:narrower C2024A00059:101 ;
    skos:prefLabel "Item I105"@en-AU ;
    dcat:accessURL <https://www.legislation.gov.au/C2024A00059/asmade/2024-07-09/text/original/epub/OEBPS/document_1/document_1.html#_Toc171508660> ;
    dcat:landingPage "https://www.legislation.gov.au/C2024A00059/asmade/2024-07-09/text/original/epub/OEBPS/document_1/document_1.html#_Toc171508660"^^xsd:anyURI ;
    dcat:theme legcons:Item .

C2024A00059:106 a legcons:Item,
        owl:Class,
        dcat:Resource ;
    rdfs:label "Item - I106 72  Disclosure to persons holding an approval"@en-AU ;
    dct:isPartOf C2024A00059:101 ;
    dct:isReferencedBy C2024A00059: ;
    rdfs:comment "72  Disclosure to persons holding an approval - Abrievated Graph Key: I106"@en-AU ;
    skos:definition "72  Disclosure to persons holding an approval"@en-AU ;
    skos:narrower C2024A00059:101 ;
    skos:prefLabel "Item I106"@en-AU ;
    dcat:accessURL <https://www.legislation.gov.au/C2024A00059/asmade/2024-07-09/text/original/epub/OEBPS/document_1/document_1.html#_Toc171508661> ;
    dcat:landingPage "https://www.legislation.gov.au/C2024A00059/asmade/2024-07-09/text/original/epub/OEBPS/document_1/document_1.html#_Toc171508661"^^xsd:anyURI ;
    dcat:theme legcons:Item .

C2024A00059:107 a legcons:Item,
        owl:Class,
        dcat:Resource ;
    rdfs:label "Item - I107 73  Disclosure for the purposes of law enforcement"@en-AU ;
    dct:isPartOf C2024A00059:101 ;
    dct:isReferencedBy C2024A00059: ;
    rdfs:comment "73  Disclosure for the purposes of law enforcement - Abrievated Graph Key: I107"@en-AU ;
    skos:definition "73  Disclosure for the purposes of law enforcement"@en-AU ;
    skos:narrower C2024A00059:101 ;
    skos:prefLabel "Item I107"@en-AU ;
    dcat:accessURL <https://www.legislation.gov.au/C2024A00059/asmade/2024-07-09/text/original/epub/OEBPS/document_1/document_1.html#_Toc171508662> ;
    dcat:landingPage "https://www.legislation.gov.au/C2024A00059/asmade/2024-07-09/text/original/epub/OEBPS/document_1/document_1.html#_Toc171508662"^^xsd:anyURI ;
    dcat:theme legcons:Item .

C2024A00059:108 a legcons:Item,
        owl:Class,
        dcat:Resource ;
    rdfs:label "Item - I108 74  Disclosure to a court tribunal etc"@en-AU ;
    dct:isPartOf C2024A00059:101 ;
    dct:isReferencedBy C2024A00059: ;
    rdfs:comment "74  Disclosure to a court tribunal etc - Abrievated Graph Key: I108"@en-AU ;
    skos:definition "74  Disclosure to a court tribunal etc"@en-AU ;
    skos:narrower C2024A00059:101 ;
    skos:prefLabel "Item I108"@en-AU ;
    dcat:accessURL <https://www.legislation.gov.au/C2024A00059/asmade/2024-07-09/text/original/epub/OEBPS/document_1/document_1.html#_Toc171508663> ;
    dcat:landingPage "https://www.legislation.gov.au/C2024A00059/asmade/2024-07-09/text/original/epub/OEBPS/document_1/document_1.html#_Toc171508663"^^xsd:anyURI ;
    dcat:theme legcons:Item .

C2024A00059:109 a legcons:Item,
        owl:Class,
        dcat:Resource ;
    rdfs:label "Item - I109 75  Use or disclosure of statistics"@en-AU ;
    dct:isPartOf C2024A00059:101 ;
    dct:isReferencedBy C2024A00059: ;
    rdfs:comment "75  Use or disclosure of statistics - Abrievated Graph Key: I109"@en-AU ;
    skos:definition "75  Use or disclosure of statistics"@en-AU ;
    skos:narrower C2024A00059:101 ;
    skos:prefLabel "Item I109"@en-AU ;
    dcat:accessURL <https://www.legislation.gov.au/C2024A00059/asmade/2024-07-09/text/original/epub/OEBPS/document_1/document_1.html#_Toc171508664> ;
    dcat:landingPage "https://www.legislation.gov.au/C2024A00059/asmade/2024-07-09/text/original/epub/OEBPS/document_1/document_1.html#_Toc171508664"^^xsd:anyURI ;
    dcat:theme legcons:Item .

C2024A00059:11 a legcons:Item,
        owl:Class,
        dcat:Resource ;
    rdfs:label "Item - I11 10  Definition of research and development"@en-AU ;
    dct:isPartOf C2024A00059:1 ;
    dct:isReferencedBy C2024A00059: ;
    rdfs:comment "10  Definition of research and development - Abrievated Graph Key: I11"@en-AU ;
    skos:definition "10  Definition of research and development"@en-AU ;
    skos:narrower C2024A00059:1 ;
    skos:prefLabel "Item I11"@en-AU ;
    dcat:accessURL <https://www.legislation.gov.au/C2024A00059/asmade/2024-07-09/text/original/epub/OEBPS/document_1/document_1.html#_Toc171508566> ;
    dcat:landingPage "https://www.legislation.gov.au/C2024A00059/asmade/2024-07-09/text/original/epub/OEBPS/document_1/document_1.html#_Toc171508566"^^xsd:anyURI ;
    dcat:theme legcons:Item .

C2024A00059:110 a legcons:Item,
        owl:Class,
        dcat:Resource ;
    rdfs:label "Item - I110 76  Use or disclosure of publicly available information"@en-AU ;
    dct:isPartOf C2024A00059:101 ;
    dct:isReferencedBy C2024A00059: ;
    rdfs:comment "76  Use or disclosure of publicly available information - Abrievated Graph Key: I110"@en-AU ;
    skos:definition "76  Use or disclosure of publicly available information"@en-AU ;
    skos:narrower C2024A00059:101 ;
    skos:prefLabel "Item I110"@en-AU ;
    dcat:accessURL <https://www.legislation.gov.au/C2024A00059/asmade/2024-07-09/text/original/epub/OEBPS/document_1/document_1.html#_Toc171508665> ;
    dcat:landingPage "https://www.legislation.gov.au/C2024A00059/asmade/2024-07-09/text/original/epub/OEBPS/document_1/document_1.html#_Toc171508665"^^xsd:anyURI ;
    dcat:theme legcons:Item .

C2024A00059:111 a legcons:Item,
        owl:Class,
        dcat:Resource ;
    rdfs:label "Item - I111 77  Disclosure to person to whom information relates"@en-AU ;
    dct:isPartOf C2024A00059:101 ;
    dct:isReferencedBy C2024A00059: ;
    rdfs:comment "77  Disclosure to person to whom information relates - Abrievated Graph Key: I111"@en-AU ;
    skos:definition "77  Disclosure to person to whom information relates"@en-AU ;
    skos:narrower C2024A00059:101 ;
    skos:prefLabel "Item I111"@en-AU ;
    dcat:accessURL <https://www.legislation.gov.au/C2024A00059/asmade/2024-07-09/text/original/epub/OEBPS/document_1/document_1.html#_Toc171508666> ;
    dcat:landingPage "https://www.legislation.gov.au/C2024A00059/asmade/2024-07-09/text/original/epub/OEBPS/document_1/document_1.html#_Toc171508666"^^xsd:anyURI ;
    dcat:theme legcons:Item .

C2024A00059:112 a legcons:Item,
        owl:Class,
        dcat:Resource ;
    rdfs:label "Item - I112 78  Use or disclosure with consent"@en-AU ;
    dct:isPartOf C2024A00059:101 ;
    dct:isReferencedBy C2024A00059: ;
    rdfs:comment "78  Use or disclosure with consent - Abrievated Graph Key: I112"@en-AU ;
    skos:definition "78  Use or disclosure with consent"@en-AU ;
    skos:narrower C2024A00059:101 ;
    skos:prefLabel "Item I112"@en-AU ;
    dcat:accessURL <https://www.legislation.gov.au/C2024A00059/asmade/2024-07-09/text/original/epub/OEBPS/document_1/document_1.html#_Toc171508667> ;
    dcat:landingPage "https://www.legislation.gov.au/C2024A00059/asmade/2024-07-09/text/original/epub/OEBPS/document_1/document_1.html#_Toc171508667"^^xsd:anyURI ;
    dcat:theme legcons:Item .

C2024A00059:113 a legcons:Item,
        owl:Class,
        dcat:Resource ;
    rdfs:label "Item - I113 79  Disclosure to person who provided information"@en-AU ;
    dct:isPartOf C2024A00059:101 ;
    dct:isReferencedBy C2024A00059: ;
    rdfs:comment "79  Disclosure to person who provided information - Abrievated Graph Key: I113"@en-AU ;
    skos:definition "79  Disclosure to person who provided information"@en-AU ;
    skos:narrower C2024A00059:101 ;
    skos:prefLabel "Item I113"@en-AU ;
    dcat:accessURL <https://www.legislation.gov.au/C2024A00059/asmade/2024-07-09/text/original/epub/OEBPS/document_1/document_1.html#_Toc171508668> ;
    dcat:landingPage "https://www.legislation.gov.au/C2024A00059/asmade/2024-07-09/text/original/epub/OEBPS/document_1/document_1.html#_Toc171508668"^^xsd:anyURI ;
    dcat:theme legcons:Item .

C2024A00059:114 a legcons:Item,
        owl:Class,
        dcat:Resource ;
    rdfs:label "Item - I114 80  Use or disclosure authorised by rules"@en-AU ;
    dct:isPartOf C2024A00059:101 ;
    dct:isReferencedBy C2024A00059: ;
    rdfs:comment "80  Use or disclosure authorised by rules - Abrievated Graph Key: I114"@en-AU ;
    skos:definition "80  Use or disclosure authorised by rules"@en-AU ;
    skos:narrower C2024A00059:101 ;
    skos:prefLabel "Item I114"@en-AU ;
    dcat:accessURL <https://www.legislation.gov.au/C2024A00059/asmade/2024-07-09/text/original/epub/OEBPS/document_1/document_1.html#_Toc171508669> ;
    dcat:landingPage "https://www.legislation.gov.au/C2024A00059/asmade/2024-07-09/text/original/epub/OEBPS/document_1/document_1.html#_Toc171508669"^^xsd:anyURI ;
    dcat:theme legcons:Item .

C2024A00059:116 a legcons:Item,
        owl:Class,
        dcat:Resource ;
    rdfs:label "Item - I116 81  Offence and civil penaltyuse or disclosure of protected information"@en-AU ;
    dct:isPartOf C2024A00059:115 ;
    dct:isReferencedBy C2024A00059: ;
    rdfs:comment "81  Offence and civil penaltyuse or disclosure of protected information - Abrievated Graph Key: I116"@en-AU ;
    skos:definition "81  Offence and civil penaltyuse or disclosure of protected information"@en-AU ;
    skos:narrower C2024A00059:115 ;
    skos:prefLabel "Item I116"@en-AU ;
    dcat:accessURL <https://www.legislation.gov.au/C2024A00059/asmade/2024-07-09/text/original/epub/OEBPS/document_1/document_1.html#_Toc171508671> ;
    dcat:landingPage "https://www.legislation.gov.au/C2024A00059/asmade/2024-07-09/text/original/epub/OEBPS/document_1/document_1.html#_Toc171508671"^^xsd:anyURI ;
    dcat:theme legcons:Item .

C2024A00059:117 a legcons:Item,
        owl:Class,
        dcat:Resource ;
    rdfs:label "Item - I117 82  Enforcement of civil penalty provisions"@en-AU ;
    dct:isPartOf C2024A00059:115 ;
    dct:isReferencedBy C2024A00059: ;
    rdfs:comment "82  Enforcement of civil penalty provisions - Abrievated Graph Key: I117"@en-AU ;
    skos:definition "82  Enforcement of civil penalty provisions"@en-AU ;
    skos:narrower C2024A00059:115 ;
    skos:prefLabel "Item I117"@en-AU ;
    dcat:accessURL <https://www.legislation.gov.au/C2024A00059/asmade/2024-07-09/text/original/epub/OEBPS/document_1/document_1.html#_Toc171508672> ;
    dcat:landingPage "https://www.legislation.gov.au/C2024A00059/asmade/2024-07-09/text/original/epub/OEBPS/document_1/document_1.html#_Toc171508672"^^xsd:anyURI ;
    dcat:theme legcons:Item .

C2024A00059:12 a legcons:Item,
        owl:Class,
        dcat:Resource ;
    rdfs:label "Item - I12 11  Act binds Crown"@en-AU ;
    dct:isPartOf C2024A00059:1 ;
    dct:isReferencedBy C2024A00059: ;
    rdfs:comment "11  Act binds Crown - Abrievated Graph Key: I12"@en-AU ;
    skos:definition "11  Act binds Crown"@en-AU ;
    skos:narrower C2024A00059:1 ;
    skos:prefLabel "Item I12"@en-AU ;
    dcat:accessURL <https://www.legislation.gov.au/C2024A00059/asmade/2024-07-09/text/original/epub/OEBPS/document_1/document_1.html#_Toc171508567> ;
    dcat:landingPage "https://www.legislation.gov.au/C2024A00059/asmade/2024-07-09/text/original/epub/OEBPS/document_1/document_1.html#_Toc171508567"^^xsd:anyURI ;
    dcat:theme legcons:Item .

C2024A00059:120 a legcons:Item,
        owl:Class,
        dcat:Resource ;
    rdfs:label "Item - I120 83  Simplified outline of this Part"@en-AU ;
    dct:isPartOf C2024A00059:119 ;
    dct:isReferencedBy C2024A00059: ;
    rdfs:comment "83  Simplified outline of this Part - Abrievated Graph Key: I120"@en-AU ;
    skos:definition "83  Simplified outline of this Part"@en-AU ;
    skos:narrower C2024A00059:119 ;
    skos:prefLabel "Item I120"@en-AU ;
    dcat:accessURL <https://www.legislation.gov.au/C2024A00059/asmade/2024-07-09/text/original/epub/OEBPS/document_1/document_1.html#_Toc171508675> ;
    dcat:landingPage "https://www.legislation.gov.au/C2024A00059/asmade/2024-07-09/text/original/epub/OEBPS/document_1/document_1.html#_Toc171508675"^^xsd:anyURI ;
    dcat:theme legcons:Item .

C2024A00059:122 a legcons:Item,
        owl:Class,
        dcat:Resource ;
    rdfs:label "Item - I122 84  Internal reconsideration of decisions"@en-AU ;
    dct:isPartOf C2024A00059:121 ;
    dct:isReferencedBy C2024A00059: ;
    rdfs:comment "84  Internal reconsideration of decisions - Abrievated Graph Key: I122"@en-AU ;
    skos:definition "84  Internal reconsideration of decisions"@en-AU ;
    skos:narrower C2024A00059:121 ;
    skos:prefLabel "Item I122"@en-AU ;
    dcat:accessURL <https://www.legislation.gov.au/C2024A00059/asmade/2024-07-09/text/original/epub/OEBPS/document_1/document_1.html#_Toc171508677> ;
    dcat:landingPage "https://www.legislation.gov.au/C2024A00059/asmade/2024-07-09/text/original/epub/OEBPS/document_1/document_1.html#_Toc171508677"^^xsd:anyURI ;
    dcat:theme legcons:Item .

C2024A00059:123 a legcons:Item,
        owl:Class,
        dcat:Resource ;
    rdfs:label "Item - I123 85  Administrative Appeals Tribunal review of decisions"@en-AU ;
    dct:isPartOf C2024A00059:121 ;
    dct:isReferencedBy C2024A00059: ;
    rdfs:comment "85  Administrative Appeals Tribunal review of decisions - Abrievated Graph Key: I123"@en-AU ;
    skos:definition "85  Administrative Appeals Tribunal review of decisions"@en-AU ;
    skos:narrower C2024A00059:121 ;
    skos:prefLabel "Item I123"@en-AU ;
    dcat:accessURL <https://www.legislation.gov.au/C2024A00059/asmade/2024-07-09/text/original/epub/OEBPS/document_1/document_1.html#_Toc171508678> ;
    dcat:landingPage "https://www.legislation.gov.au/C2024A00059/asmade/2024-07-09/text/original/epub/OEBPS/document_1/document_1.html#_Toc171508678"^^xsd:anyURI ;
    dcat:theme legcons:Item .

C2024A00059:125 a legcons:Item,
        owl:Class,
        dcat:Resource ;
    rdfs:label "Item - I125 86  Recoverable payments"@en-AU ;
    dct:isPartOf C2024A00059:124 ;
    dct:isReferencedBy C2024A00059: ;
    rdfs:comment "86  Recoverable payments - Abrievated Graph Key: I125"@en-AU ;
    skos:definition "86  Recoverable payments"@en-AU ;
    skos:narrower C2024A00059:124 ;
    skos:prefLabel "Item I125"@en-AU ;
    dcat:accessURL <https://www.legislation.gov.au/C2024A00059/asmade/2024-07-09/text/original/epub/OEBPS/document_1/document_1.html#_Toc171508680> ;
    dcat:landingPage "https://www.legislation.gov.au/C2024A00059/asmade/2024-07-09/text/original/epub/OEBPS/document_1/document_1.html#_Toc171508680"^^xsd:anyURI ;
    dcat:theme legcons:Item .

C2024A00059:126 a legcons:Item,
        owl:Class,
        dcat:Resource ;
    rdfs:label "Item - I126 87  Report about recoverable payments"@en-AU ;
    dct:isPartOf C2024A00059:124 ;
    dct:isReferencedBy C2024A00059: ;
    rdfs:comment "87  Report about recoverable payments - Abrievated Graph Key: I126"@en-AU ;
    skos:definition "87  Report about recoverable payments"@en-AU ;
    skos:narrower C2024A00059:124 ;
    skos:prefLabel "Item I126"@en-AU ;
    dcat:accessURL <https://www.legislation.gov.au/C2024A00059/asmade/2024-07-09/text/original/epub/OEBPS/document_1/document_1.html#_Toc171508681> ;
    dcat:landingPage "https://www.legislation.gov.au/C2024A00059/asmade/2024-07-09/text/original/epub/OEBPS/document_1/document_1.html#_Toc171508681"^^xsd:anyURI ;
    dcat:theme legcons:Item .

C2024A00059:128 a legcons:Item,
        owl:Class,
        dcat:Resource ;
    rdfs:label "Item - I128 88  Delegation by Minister"@en-AU ;
    dct:isPartOf C2024A00059:127 ;
    dct:isReferencedBy C2024A00059: ;
    rdfs:comment "88  Delegation by Minister - Abrievated Graph Key: I128"@en-AU ;
    skos:definition "88  Delegation by Minister"@en-AU ;
    skos:narrower C2024A00059:127 ;
    skos:prefLabel "Item I128"@en-AU ;
    dcat:accessURL <https://www.legislation.gov.au/C2024A00059/asmade/2024-07-09/text/original/epub/OEBPS/document_1/document_1.html#_Toc171508683> ;
    dcat:landingPage "https://www.legislation.gov.au/C2024A00059/asmade/2024-07-09/text/original/epub/OEBPS/document_1/document_1.html#_Toc171508683"^^xsd:anyURI ;
    dcat:theme legcons:Item .

C2024A00059:129 a legcons:Item,
        owl:Class,
        dcat:Resource ;
    rdfs:label "Item - I129 89  Delegation by Secretary"@en-AU ;
    dct:isPartOf C2024A00059:127 ;
    dct:isReferencedBy C2024A00059: ;
    rdfs:comment "89  Delegation by Secretary - Abrievated Graph Key: I129"@en-AU ;
    skos:definition "89  Delegation by Secretary"@en-AU ;
    skos:narrower C2024A00059:127 ;
    skos:prefLabel "Item I129"@en-AU ;
    dcat:accessURL <https://www.legislation.gov.au/C2024A00059/asmade/2024-07-09/text/original/epub/OEBPS/document_1/document_1.html#_Toc171508684> ;
    dcat:landingPage "https://www.legislation.gov.au/C2024A00059/asmade/2024-07-09/text/original/epub/OEBPS/document_1/document_1.html#_Toc171508684"^^xsd:anyURI ;
    dcat:theme legcons:Item .

C2024A00059:13 a legcons:Item,
        owl:Class,
        dcat:Resource ;
    rdfs:label "Item - I13 12  Extension of this Act to external Territories"@en-AU ;
    dct:isPartOf C2024A00059:1 ;
    dct:isReferencedBy C2024A00059: ;
    rdfs:comment "12  Extension of this Act to external Territories - Abrievated Graph Key: I13"@en-AU ;
    skos:definition "12  Extension of this Act to external Territories"@en-AU ;
    skos:narrower C2024A00059:1 ;
    skos:prefLabel "Item I13"@en-AU ;
    dcat:accessURL <https://www.legislation.gov.au/C2024A00059/asmade/2024-07-09/text/original/epub/OEBPS/document_1/document_1.html#_Toc171508568> ;
    dcat:landingPage "https://www.legislation.gov.au/C2024A00059/asmade/2024-07-09/text/original/epub/OEBPS/document_1/document_1.html#_Toc171508568"^^xsd:anyURI ;
    dcat:theme legcons:Item .

C2024A00059:130 a legcons:Item,
        owl:Class,
        dcat:Resource ;
    rdfs:label "Item - I130 90  Rules"@en-AU ;
    dct:isPartOf C2024A00059:127 ;
    dct:isReferencedBy C2024A00059: ;
    rdfs:comment "90  Rules - Abrievated Graph Key: I130"@en-AU ;
    skos:definition "90  Rules"@en-AU ;
    skos:narrower C2024A00059:127 ;
    skos:prefLabel "Item I130"@en-AU ;
    dcat:accessURL <https://www.legislation.gov.au/C2024A00059/asmade/2024-07-09/text/original/epub/OEBPS/document_1/document_1.html#_Toc171508685> ;
    dcat:landingPage "https://www.legislation.gov.au/C2024A00059/asmade/2024-07-09/text/original/epub/OEBPS/document_1/document_1.html#_Toc171508685"^^xsd:anyURI ;
    dcat:theme legcons:Item .

C2024A00059:14 a legcons:Item,
        owl:Class,
        dcat:Resource ;
    rdfs:label "Item - I14 13  Extra territorial application of this Act"@en-AU ;
    dct:isPartOf C2024A00059:1 ;
    dct:isReferencedBy C2024A00059: ;
    rdfs:comment "13  Extra territorial application of this Act - Abrievated Graph Key: I14"@en-AU ;
    skos:definition "13  Extra territorial application of this Act"@en-AU ;
    skos:narrower C2024A00059:1 ;
    skos:prefLabel "Item I14"@en-AU ;
    dcat:accessURL <https://www.legislation.gov.au/C2024A00059/asmade/2024-07-09/text/original/epub/OEBPS/document_1/document_1.html#_Toc171508569> ;
    dcat:landingPage "https://www.legislation.gov.au/C2024A00059/asmade/2024-07-09/text/original/epub/OEBPS/document_1/document_1.html#_Toc171508569"^^xsd:anyURI ;
    dcat:theme legcons:Item .

C2024A00059:17 a legcons:Item,
        owl:Class,
        dcat:Resource ;
    rdfs:label "Item - I17 14  Simplified outline of this Part"@en-AU ;
    dct:isPartOf C2024A00059:16 ;
    dct:isReferencedBy C2024A00059: ;
    rdfs:comment "14  Simplified outline of this Part - Abrievated Graph Key: I17"@en-AU ;
    skos:definition "14  Simplified outline of this Part"@en-AU ;
    skos:narrower C2024A00059:16 ;
    skos:prefLabel "Item I17"@en-AU ;
    dcat:accessURL <https://www.legislation.gov.au/C2024A00059/asmade/2024-07-09/text/original/epub/OEBPS/document_1/document_1.html#_Toc171508572> ;
    dcat:landingPage "https://www.legislation.gov.au/C2024A00059/asmade/2024-07-09/text/original/epub/OEBPS/document_1/document_1.html#_Toc171508572"^^xsd:anyURI ;
    dcat:theme legcons:Item .

C2024A00059:18 a legcons:Division,
        owl:Class,
        dcat:Resource ;
    rdfs:label "Division - D18 Division 2 Levy or charge payments"@en-AU ;
    dct:isPartOf C2024A00059:15 ;
    dct:isReferencedBy C2024A00059: ;
    rdfs:comment "Division 2 Levy or charge payments - Abrievated Graph Key: D18"@en-AU ;
    skos:definition "Division 2 Levy or charge payments"@en-AU ;
    skos:narrower C2024A00059:15 ;
    skos:prefLabel "Division D18"@en-AU ;
    dcat:accessURL <https://www.legislation.gov.au/C2024A00059/asmade/2024-07-09/text/original/epub/OEBPS/document_1/document_1.html#_Toc171508573> ;
    dcat:landingPage "https://www.legislation.gov.au/C2024A00059/asmade/2024-07-09/text/original/epub/OEBPS/document_1/document_1.html#_Toc171508573"^^xsd:anyURI ;
    dcat:theme legcons:Division .

C2024A00059:2 a legcons:Item,
        owl:Class,
        dcat:Resource ;
    rdfs:label "Item - I2 1  Short title"@en-AU ;
    dct:isPartOf C2024A00059:1 ;
    dct:isReferencedBy C2024A00059: ;
    rdfs:comment "1  Short title - Abrievated Graph Key: I2"@en-AU ;
    skos:definition "1  Short title"@en-AU ;
    skos:narrower C2024A00059:1 ;
    skos:prefLabel "Item I2"@en-AU ;
    dcat:accessURL <https://www.legislation.gov.au/C2024A00059/asmade/2024-07-09/text/original/epub/OEBPS/document_1/document_1.html#_Toc171508557> ;
    dcat:landingPage "https://www.legislation.gov.au/C2024A00059/asmade/2024-07-09/text/original/epub/OEBPS/document_1/document_1.html#_Toc171508557"^^xsd:anyURI ;
    dcat:theme legcons:Item .

C2024A00059:20 a legcons:Item,
        owl:Class,
        dcat:Resource ;
    rdfs:label "Item - I20 15  Commonwealth to make levy or charge payments"@en-AU ;
    dct:isPartOf C2024A00059:19 ;
    dct:isReferencedBy C2024A00059: ;
    rdfs:comment "15  Commonwealth to make levy or charge payments - Abrievated Graph Key: I20"@en-AU ;
    skos:definition "15  Commonwealth to make levy or charge payments"@en-AU ;
    skos:narrower C2024A00059:19 ;
    skos:prefLabel "Item I20"@en-AU ;
    dcat:accessURL <https://www.legislation.gov.au/C2024A00059/asmade/2024-07-09/text/original/epub/OEBPS/document_1/document_1.html#_Toc171508575> ;
    dcat:landingPage "https://www.legislation.gov.au/C2024A00059/asmade/2024-07-09/text/original/epub/OEBPS/document_1/document_1.html#_Toc171508575"^^xsd:anyURI ;
    dcat:theme legcons:Item .

C2024A00059:21 a legcons:Item,
        owl:Class,
        dcat:Resource ;
    rdfs:label "Item - I21 16  Payment of Commonwealth costs"@en-AU ;
    dct:isPartOf C2024A00059:19 ;
    dct:isReferencedBy C2024A00059: ;
    rdfs:comment "16  Payment of Commonwealth costs - Abrievated Graph Key: I21"@en-AU ;
    skos:definition "16  Payment of Commonwealth costs"@en-AU ;
    skos:narrower C2024A00059:19 ;
    skos:prefLabel "Item I21"@en-AU ;
    dcat:accessURL <https://www.legislation.gov.au/C2024A00059/asmade/2024-07-09/text/original/epub/OEBPS/document_1/document_1.html#_Toc171508576> ;
    dcat:landingPage "https://www.legislation.gov.au/C2024A00059/asmade/2024-07-09/text/original/epub/OEBPS/document_1/document_1.html#_Toc171508576"^^xsd:anyURI ;
    dcat:theme legcons:Item .

C2024A00059:22 a legcons:Item,
        owl:Class,
        dcat:Resource ;
    rdfs:label "Item - I22 17  Effect of refunds"@en-AU ;
    dct:isPartOf C2024A00059:19 ;
    dct:isReferencedBy C2024A00059: ;
    rdfs:comment "17  Effect of refunds - Abrievated Graph Key: I22"@en-AU ;
    skos:definition "17  Effect of refunds"@en-AU ;
    skos:narrower C2024A00059:19 ;
    skos:prefLabel "Item I22"@en-AU ;
    dcat:accessURL <https://www.legislation.gov.au/C2024A00059/asmade/2024-07-09/text/original/epub/OEBPS/document_1/document_1.html#_Toc171508577> ;
    dcat:landingPage "https://www.legislation.gov.au/C2024A00059/asmade/2024-07-09/text/original/epub/OEBPS/document_1/document_1.html#_Toc171508577"^^xsd:anyURI ;
    dcat:theme legcons:Item .

C2024A00059:23 a legcons:Subdivision,
        owl:Class,
        dcat:Resource ;
    rdfs:label "Subdivision - S23 Subdivision BSpending requirements for declared recipient bodies"@en-AU ;
    dct:isPartOf C2024A00059:15 ;
    dct:isReferencedBy C2024A00059: ;
    rdfs:comment "Subdivision BSpending requirements for declared recipient bodies - Abrievated Graph Key: S23"@en-AU ;
    skos:definition "Subdivision BSpending requirements for declared recipient bodies"@en-AU ;
    skos:narrower C2024A00059:15 ;
    skos:prefLabel "Subdivision S23"@en-AU ;
    dcat:accessURL <https://www.legislation.gov.au/C2024A00059/asmade/2024-07-09/text/original/epub/OEBPS/document_1/document_1.html#_Toc171508578> ;
    dcat:landingPage "https://www.legislation.gov.au/C2024A00059/asmade/2024-07-09/text/original/epub/OEBPS/document_1/document_1.html#_Toc171508578"^^xsd:anyURI ;
    dcat:theme legcons:Subdivision .

C2024A00059:24 a legcons:Item,
        owl:Class,
        dcat:Resource ;
    rdfs:label "Item - I24 18  Spending of amounts equal to marketing collected amounts"@en-AU ;
    dct:isPartOf C2024A00059:15 ;
    dct:isReferencedBy C2024A00059: ;
    rdfs:comment "18  Spending of amounts equal to marketing collected amounts - Abrievated Graph Key: I24"@en-AU ;
    skos:definition "18  Spending of amounts equal to marketing collected amounts"@en-AU ;
    skos:narrower C2024A00059:15 ;
    skos:prefLabel "Item I24"@en-AU ;
    dcat:accessURL <https://www.legislation.gov.au/C2024A00059/asmade/2024-07-09/text/original/epub/OEBPS/document_1/document_1.html#_Toc171508579> ;
    dcat:landingPage "https://www.legislation.gov.au/C2024A00059/asmade/2024-07-09/text/original/epub/OEBPS/document_1/document_1.html#_Toc171508579"^^xsd:anyURI ;
    dcat:theme legcons:Item .

C2024A00059:25 a legcons:Item,
        owl:Class,
        dcat:Resource ;
    rdfs:label "Item - I25 19  Spending of amounts equal to research and development collected amounts"@en-AU ;
    dct:isPartOf C2024A00059:15 ;
    dct:isReferencedBy C2024A00059: ;
    rdfs:comment "19  Spending of amounts equal to research and development collected amounts - Abrievated Graph Key: I25"@en-AU ;
    skos:definition "19  Spending of amounts equal to research and development collected amounts"@en-AU ;
    skos:narrower C2024A00059:15 ;
    skos:prefLabel "Item I25"@en-AU ;
    dcat:accessURL <https://www.legislation.gov.au/C2024A00059/asmade/2024-07-09/text/original/epub/OEBPS/document_1/document_1.html#_Toc171508580> ;
    dcat:landingPage "https://www.legislation.gov.au/C2024A00059/asmade/2024-07-09/text/original/epub/OEBPS/document_1/document_1.html#_Toc171508580"^^xsd:anyURI ;
    dcat:theme legcons:Item .

C2024A00059:26 a legcons:Item,
        owl:Class,
        dcat:Resource ;
    rdfs:label "Item - I26 20  Spending of amounts equal to general collected amounts"@en-AU ;
    dct:isPartOf C2024A00059:15 ;
    dct:isReferencedBy C2024A00059: ;
    rdfs:comment "20  Spending of amounts equal to general collected amounts - Abrievated Graph Key: I26"@en-AU ;
    skos:definition "20  Spending of amounts equal to general collected amounts"@en-AU ;
    skos:narrower C2024A00059:15 ;
    skos:prefLabel "Item I26"@en-AU ;
    dcat:accessURL <https://www.legislation.gov.au/C2024A00059/asmade/2024-07-09/text/original/epub/OEBPS/document_1/document_1.html#_Toc171508581> ;
    dcat:landingPage "https://www.legislation.gov.au/C2024A00059/asmade/2024-07-09/text/original/epub/OEBPS/document_1/document_1.html#_Toc171508581"^^xsd:anyURI ;
    dcat:theme legcons:Item .

C2024A00059:27 a legcons:Subdivision,
        owl:Class,
        dcat:Resource ;
    rdfs:label "Subdivision - S27 Subdivision CSpending requirements for statutory recipient bodies"@en-AU ;
    dct:isPartOf C2024A00059:15 ;
    dct:isReferencedBy C2024A00059: ;
    rdfs:comment "Subdivision CSpending requirements for statutory recipient bodies - Abrievated Graph Key: S27"@en-AU ;
    skos:definition "Subdivision CSpending requirements for statutory recipient bodies"@en-AU ;
    skos:narrower C2024A00059:15 ;
    skos:prefLabel "Subdivision S27"@en-AU ;
    dcat:accessURL <https://www.legislation.gov.au/C2024A00059/asmade/2024-07-09/text/original/epub/OEBPS/document_1/document_1.html#_Toc171508582> ;
    dcat:landingPage "https://www.legislation.gov.au/C2024A00059/asmade/2024-07-09/text/original/epub/OEBPS/document_1/document_1.html#_Toc171508582"^^xsd:anyURI ;
    dcat:theme legcons:Subdivision .

C2024A00059:28 a legcons:Item,
        owl:Class,
        dcat:Resource ;
    rdfs:label "Item - I28 21  Spending of amounts equal to marketing collected amounts"@en-AU ;
    dct:isPartOf C2024A00059:15 ;
    dct:isReferencedBy C2024A00059: ;
    rdfs:comment "21  Spending of amounts equal to marketing collected amounts - Abrievated Graph Key: I28"@en-AU ;
    skos:definition "21  Spending of amounts equal to marketing collected amounts"@en-AU ;
    skos:narrower C2024A00059:15 ;
    skos:prefLabel "Item I28"@en-AU ;
    dcat:accessURL <https://www.legislation.gov.au/C2024A00059/asmade/2024-07-09/text/original/epub/OEBPS/document_1/document_1.html#_Toc171508583> ;
    dcat:landingPage "https://www.legislation.gov.au/C2024A00059/asmade/2024-07-09/text/original/epub/OEBPS/document_1/document_1.html#_Toc171508583"^^xsd:anyURI ;
    dcat:theme legcons:Item .

C2024A00059:29 a legcons:Item,
        owl:Class,
        dcat:Resource ;
    rdfs:label "Item - I29 22  Spending of amounts equal to research and development collected amounts"@en-AU ;
    dct:isPartOf C2024A00059:15 ;
    dct:isReferencedBy C2024A00059: ;
    rdfs:comment "22  Spending of amounts equal to research and development collected amounts - Abrievated Graph Key: I29"@en-AU ;
    skos:definition "22  Spending of amounts equal to research and development collected amounts"@en-AU ;
    skos:narrower C2024A00059:15 ;
    skos:prefLabel "Item I29"@en-AU ;
    dcat:accessURL <https://www.legislation.gov.au/C2024A00059/asmade/2024-07-09/text/original/epub/OEBPS/document_1/document_1.html#_Toc171508584> ;
    dcat:landingPage "https://www.legislation.gov.au/C2024A00059/asmade/2024-07-09/text/original/epub/OEBPS/document_1/document_1.html#_Toc171508584"^^xsd:anyURI ;
    dcat:theme legcons:Item .

C2024A00059:3 a legcons:Item,
        owl:Class,
        dcat:Resource ;
    rdfs:label "Item - I3 2  Commencement"@en-AU ;
    dct:isPartOf C2024A00059:1 ;
    dct:isReferencedBy C2024A00059: ;
    rdfs:comment "2  Commencement - Abrievated Graph Key: I3"@en-AU ;
    skos:definition "2  Commencement"@en-AU ;
    skos:narrower C2024A00059:1 ;
    skos:prefLabel "Item I3"@en-AU ;
    dcat:accessURL <https://www.legislation.gov.au/C2024A00059/asmade/2024-07-09/text/original/epub/OEBPS/document_1/document_1.html#_Toc171508558> ;
    dcat:landingPage "https://www.legislation.gov.au/C2024A00059/asmade/2024-07-09/text/original/epub/OEBPS/document_1/document_1.html#_Toc171508558"^^xsd:anyURI ;
    dcat:theme legcons:Item .

C2024A00059:30 a legcons:Division,
        owl:Class,
        dcat:Resource ;
    rdfs:label "Division - D30 Division 3 Matching payments"@en-AU ;
    dct:isPartOf C2024A00059:15 ;
    dct:isReferencedBy C2024A00059: ;
    rdfs:comment "Division 3 Matching payments - Abrievated Graph Key: D30"@en-AU ;
    skos:definition "Division 3 Matching payments"@en-AU ;
    skos:narrower C2024A00059:15 ;
    skos:prefLabel "Division D30"@en-AU ;
    dcat:accessURL <https://www.legislation.gov.au/C2024A00059/asmade/2024-07-09/text/original/epub/OEBPS/document_1/document_1.html#_Toc171508585> ;
    dcat:landingPage "https://www.legislation.gov.au/C2024A00059/asmade/2024-07-09/text/original/epub/OEBPS/document_1/document_1.html#_Toc171508585"^^xsd:anyURI ;
    dcat:theme legcons:Division .

C2024A00059:31 a legcons:Subdivision,
        owl:Class,
        dcat:Resource ;
    rdfs:label "Subdivision - S31 Subdivision ACommonwealth to make matching payments to most recipient bodies"@en-AU ;
    dct:isPartOf C2024A00059:15 ;
    dct:isReferencedBy C2024A00059: ;
    rdfs:comment "Subdivision ACommonwealth to make matching payments to most recipient bodies - Abrievated Graph Key: S31"@en-AU ;
    skos:definition "Subdivision ACommonwealth to make matching payments to most recipient bodies"@en-AU ;
    skos:narrower C2024A00059:15 ;
    skos:prefLabel "Subdivision S31"@en-AU ;
    dcat:accessURL <https://www.legislation.gov.au/C2024A00059/asmade/2024-07-09/text/original/epub/OEBPS/document_1/document_1.html#_Toc171508586> ;
    dcat:landingPage "https://www.legislation.gov.au/C2024A00059/asmade/2024-07-09/text/original/epub/OEBPS/document_1/document_1.html#_Toc171508586"^^xsd:anyURI ;
    dcat:theme legcons:Subdivision .

C2024A00059:32 a legcons:Item,
        owl:Class,
        dcat:Resource ;
    rdfs:label "Item - I32 23  Commonwealth to make matching payments"@en-AU ;
    dct:isPartOf C2024A00059:15 ;
    dct:isReferencedBy C2024A00059: ;
    rdfs:comment "23  Commonwealth to make matching payments - Abrievated Graph Key: I32"@en-AU ;
    skos:definition "23  Commonwealth to make matching payments"@en-AU ;
    skos:narrower C2024A00059:15 ;
    skos:prefLabel "Item I32"@en-AU ;
    dcat:accessURL <https://www.legislation.gov.au/C2024A00059/asmade/2024-07-09/text/original/epub/OEBPS/document_1/document_1.html#_Toc171508587> ;
    dcat:landingPage "https://www.legislation.gov.au/C2024A00059/asmade/2024-07-09/text/original/epub/OEBPS/document_1/document_1.html#_Toc171508587"^^xsd:anyURI ;
    dcat:theme legcons:Item .

C2024A00059:33 a legcons:Item,
        owl:Class,
        dcat:Resource ;
    rdfs:label "Item - I33 24  Definition of qualifying expenditure amount"@en-AU ;
    dct:isPartOf C2024A00059:15 ;
    dct:isReferencedBy C2024A00059: ;
    rdfs:comment "24  Definition of qualifying expenditure amount - Abrievated Graph Key: I33"@en-AU ;
    skos:definition "24  Definition of qualifying expenditure amount"@en-AU ;
    skos:narrower C2024A00059:15 ;
    skos:prefLabel "Item I33"@en-AU ;
    dcat:accessURL <https://www.legislation.gov.au/C2024A00059/asmade/2024-07-09/text/original/epub/OEBPS/document_1/document_1.html#_Toc171508588> ;
    dcat:landingPage "https://www.legislation.gov.au/C2024A00059/asmade/2024-07-09/text/original/epub/OEBPS/document_1/document_1.html#_Toc171508588"^^xsd:anyURI ;
    dcat:theme legcons:Item .

C2024A00059:34 a legcons:Item,
        owl:Class,
        dcat:Resource ;
    rdfs:label "Item - I34 25  Definition of average gross value of production amount"@en-AU ;
    dct:isPartOf C2024A00059:15 ;
    dct:isReferencedBy C2024A00059: ;
    rdfs:comment "25  Definition of average gross value of production amount - Abrievated Graph Key: I34"@en-AU ;
    skos:definition "25  Definition of average gross value of production amount"@en-AU ;
    skos:narrower C2024A00059:15 ;
    skos:prefLabel "Item I34"@en-AU ;
    dcat:accessURL <https://www.legislation.gov.au/C2024A00059/asmade/2024-07-09/text/original/epub/OEBPS/document_1/document_1.html#_Toc171508589> ;
    dcat:landingPage "https://www.legislation.gov.au/C2024A00059/asmade/2024-07-09/text/original/epub/OEBPS/document_1/document_1.html#_Toc171508589"^^xsd:anyURI ;
    dcat:theme legcons:Item .

C2024A00059:35 a legcons:Subdivision,
        owl:Class,
        dcat:Resource ;
    rdfs:label "Subdivision - S35 Subdivision BCommonwealth to make matching payments to Fisheries Research and Development Corporation"@en-AU ;
    dct:isPartOf C2024A00059:15 ;
    dct:isReferencedBy C2024A00059: ;
    rdfs:comment "Subdivision BCommonwealth to make matching payments to Fisheries Research and Development Corporation - Abrievated Graph Key: S35"@en-AU ;
    skos:definition "Subdivision BCommonwealth to make matching payments to Fisheries Research and Development Corporation"@en-AU ;
    skos:narrower C2024A00059:15 ;
    skos:prefLabel "Subdivision S35"@en-AU ;
    dcat:accessURL <https://www.legislation.gov.au/C2024A00059/asmade/2024-07-09/text/original/epub/OEBPS/document_1/document_1.html#_Toc171508590> ;
    dcat:landingPage "https://www.legislation.gov.au/C2024A00059/asmade/2024-07-09/text/original/epub/OEBPS/document_1/document_1.html#_Toc171508590"^^xsd:anyURI ;
    dcat:theme legcons:Subdivision .

C2024A00059:36 a legcons:Item,
        owl:Class,
        dcat:Resource ;
    rdfs:label "Item - I36 26  Commonwealth to make matching payments in relation to the fishing industry except declared fisheries"@en-AU ;
    dct:isPartOf C2024A00059:15 ;
    dct:isReferencedBy C2024A00059: ;
    rdfs:comment "26  Commonwealth to make matching payments in relation to the fishing industry except declared fisheries - Abrievated Graph Key: I36"@en-AU ;
    skos:definition "26  Commonwealth to make matching payments in relation to the fishing industry except declared fisheries"@en-AU ;
    skos:narrower C2024A00059:15 ;
    skos:prefLabel "Item I36"@en-AU ;
    dcat:accessURL <https://www.legislation.gov.au/C2024A00059/asmade/2024-07-09/text/original/epub/OEBPS/document_1/document_1.html#_Toc171508591> ;
    dcat:landingPage "https://www.legislation.gov.au/C2024A00059/asmade/2024-07-09/text/original/epub/OEBPS/document_1/document_1.html#_Toc171508591"^^xsd:anyURI ;
    dcat:theme legcons:Item .

C2024A00059:37 a legcons:Item,
        owl:Class,
        dcat:Resource ;
    rdfs:label "Item - I37 27  Commonwealth to make matching payments in relation to a declared fishery"@en-AU ;
    dct:isPartOf C2024A00059:15 ;
    dct:isReferencedBy C2024A00059: ;
    rdfs:comment "27  Commonwealth to make matching payments in relation to a declared fishery - Abrievated Graph Key: I37"@en-AU ;
    skos:definition "27  Commonwealth to make matching payments in relation to a declared fishery"@en-AU ;
    skos:narrower C2024A00059:15 ;
    skos:prefLabel "Item I37"@en-AU ;
    dcat:accessURL <https://www.legislation.gov.au/C2024A00059/asmade/2024-07-09/text/original/epub/OEBPS/document_1/document_1.html#_Toc171508592> ;
    dcat:landingPage "https://www.legislation.gov.au/C2024A00059/asmade/2024-07-09/text/original/epub/OEBPS/document_1/document_1.html#_Toc171508592"^^xsd:anyURI ;
    dcat:theme legcons:Item .

C2024A00059:38 a legcons:Item,
        owl:Class,
        dcat:Resource ;
    rdfs:label "Item - I38 28  Scope of Fisheries Research and Development Corporations expenditure amounts"@en-AU ;
    dct:isPartOf C2024A00059:15 ;
    dct:isReferencedBy C2024A00059: ;
    rdfs:comment "28  Scope of Fisheries Research and Development Corporations expenditure amounts - Abrievated Graph Key: I38"@en-AU ;
    skos:definition "28  Scope of Fisheries Research and Development Corporations expenditure amounts"@en-AU ;
    skos:narrower C2024A00059:15 ;
    skos:prefLabel "Item I38"@en-AU ;
    dcat:accessURL <https://www.legislation.gov.au/C2024A00059/asmade/2024-07-09/text/original/epub/OEBPS/document_1/document_1.html#_Toc171508593> ;
    dcat:landingPage "https://www.legislation.gov.au/C2024A00059/asmade/2024-07-09/text/original/epub/OEBPS/document_1/document_1.html#_Toc171508593"^^xsd:anyURI ;
    dcat:theme legcons:Item .

C2024A00059:39 a legcons:Item,
        owl:Class,
        dcat:Resource ;
    rdfs:label "Item - I39 29  Definition of average total main fishing industry GVP amount"@en-AU ;
    dct:isPartOf C2024A00059:15 ;
    dct:isReferencedBy C2024A00059: ;
    rdfs:comment "29  Definition of average total main fishing industry GVP amount - Abrievated Graph Key: I39"@en-AU ;
    skos:definition "29  Definition of average total main fishing industry GVP amount"@en-AU ;
    skos:narrower C2024A00059:15 ;
    skos:prefLabel "Item I39"@en-AU ;
    dcat:accessURL <https://www.legislation.gov.au/C2024A00059/asmade/2024-07-09/text/original/epub/OEBPS/document_1/document_1.html#_Toc171508594> ;
    dcat:landingPage "https://www.legislation.gov.au/C2024A00059/asmade/2024-07-09/text/original/epub/OEBPS/document_1/document_1.html#_Toc171508594"^^xsd:anyURI ;
    dcat:theme legcons:Item .

C2024A00059:4 a legcons:Item,
        owl:Class,
        dcat:Resource ;
    rdfs:label "Item - I4 3  Simplified outline of this Act"@en-AU ;
    dct:isPartOf C2024A00059:1 ;
    dct:isReferencedBy C2024A00059: ;
    rdfs:comment "3  Simplified outline of this Act - Abrievated Graph Key: I4"@en-AU ;
    skos:definition "3  Simplified outline of this Act"@en-AU ;
    skos:narrower C2024A00059:1 ;
    skos:prefLabel "Item I4"@en-AU ;
    dcat:accessURL <https://www.legislation.gov.au/C2024A00059/asmade/2024-07-09/text/original/epub/OEBPS/document_1/document_1.html#_Toc171508559> ;
    dcat:landingPage "https://www.legislation.gov.au/C2024A00059/asmade/2024-07-09/text/original/epub/OEBPS/document_1/document_1.html#_Toc171508559"^^xsd:anyURI ;
    dcat:theme legcons:Item .

C2024A00059:40 a legcons:Item,
        owl:Class,
        dcat:Resource ;
    rdfs:label "Item - I40 30  Definition of average Commonwealth main fishing industry GVP amount"@en-AU ;
    dct:isPartOf C2024A00059:15 ;
    dct:isReferencedBy C2024A00059: ;
    rdfs:comment "30  Definition of average Commonwealth main fishing industry GVP amount - Abrievated Graph Key: I40"@en-AU ;
    skos:definition "30  Definition of average Commonwealth main fishing industry GVP amount"@en-AU ;
    skos:narrower C2024A00059:15 ;
    skos:prefLabel "Item I40"@en-AU ;
    dcat:accessURL <https://www.legislation.gov.au/C2024A00059/asmade/2024-07-09/text/original/epub/OEBPS/document_1/document_1.html#_Toc171508595> ;
    dcat:landingPage "https://www.legislation.gov.au/C2024A00059/asmade/2024-07-09/text/original/epub/OEBPS/document_1/document_1.html#_Toc171508595"^^xsd:anyURI ;
    dcat:theme legcons:Item .

C2024A00059:41 a legcons:Item,
        owl:Class,
        dcat:Resource ;
    rdfs:label "Item - I41 31  Definition of average StateTerritory main fishing industry GVP amount"@en-AU ;
    dct:isPartOf C2024A00059:15 ;
    dct:isReferencedBy C2024A00059: ;
    rdfs:comment "31  Definition of average StateTerritory main fishing industry GVP amount - Abrievated Graph Key: I41"@en-AU ;
    skos:definition "31  Definition of average StateTerritory main fishing industry GVP amount"@en-AU ;
    skos:narrower C2024A00059:15 ;
    skos:prefLabel "Item I41"@en-AU ;
    dcat:accessURL <https://www.legislation.gov.au/C2024A00059/asmade/2024-07-09/text/original/epub/OEBPS/document_1/document_1.html#_Toc171508596> ;
    dcat:landingPage "https://www.legislation.gov.au/C2024A00059/asmade/2024-07-09/text/original/epub/OEBPS/document_1/document_1.html#_Toc171508596"^^xsd:anyURI ;
    dcat:theme legcons:Item .

C2024A00059:42 a legcons:Item,
        owl:Class,
        dcat:Resource ;
    rdfs:label "Item - I42 32  Definition of average declared fishery GVP amount"@en-AU ;
    dct:isPartOf C2024A00059:15 ;
    dct:isReferencedBy C2024A00059: ;
    rdfs:comment "32  Definition of average declared fishery GVP amount - Abrievated Graph Key: I42"@en-AU ;
    skos:definition "32  Definition of average declared fishery GVP amount"@en-AU ;
    skos:narrower C2024A00059:15 ;
    skos:prefLabel "Item I42"@en-AU ;
    dcat:accessURL <https://www.legislation.gov.au/C2024A00059/asmade/2024-07-09/text/original/epub/OEBPS/document_1/document_1.html#_Toc171508597> ;
    dcat:landingPage "https://www.legislation.gov.au/C2024A00059/asmade/2024-07-09/text/original/epub/OEBPS/document_1/document_1.html#_Toc171508597"^^xsd:anyURI ;
    dcat:theme legcons:Item .

C2024A00059:43 a legcons:Subdivision,
        owl:Class,
        dcat:Resource ;
    rdfs:label "Subdivision - S43 Subdivision CSpending requirements for declared recipient bodies"@en-AU ;
    dct:isPartOf C2024A00059:15 ;
    dct:isReferencedBy C2024A00059: ;
    rdfs:comment "Subdivision CSpending requirements for declared recipient bodies - Abrievated Graph Key: S43"@en-AU ;
    skos:definition "Subdivision CSpending requirements for declared recipient bodies"@en-AU ;
    skos:narrower C2024A00059:15 ;
    skos:prefLabel "Subdivision S43"@en-AU ;
    dcat:accessURL <https://www.legislation.gov.au/C2024A00059/asmade/2024-07-09/text/original/epub/OEBPS/document_1/document_1.html#_Toc171508598> ;
    dcat:landingPage "https://www.legislation.gov.au/C2024A00059/asmade/2024-07-09/text/original/epub/OEBPS/document_1/document_1.html#_Toc171508598"^^xsd:anyURI ;
    dcat:theme legcons:Subdivision .

C2024A00059:44 a legcons:Item,
        owl:Class,
        dcat:Resource ;
    rdfs:label "Item - I44 33  Spending of matching payments"@en-AU ;
    dct:isPartOf C2024A00059:15 ;
    dct:isReferencedBy C2024A00059: ;
    rdfs:comment "33  Spending of matching payments - Abrievated Graph Key: I44"@en-AU ;
    skos:definition "33  Spending of matching payments"@en-AU ;
    skos:narrower C2024A00059:15 ;
    skos:prefLabel "Item I44"@en-AU ;
    dcat:accessURL <https://www.legislation.gov.au/C2024A00059/asmade/2024-07-09/text/original/epub/OEBPS/document_1/document_1.html#_Toc171508599> ;
    dcat:landingPage "https://www.legislation.gov.au/C2024A00059/asmade/2024-07-09/text/original/epub/OEBPS/document_1/document_1.html#_Toc171508599"^^xsd:anyURI ;
    dcat:theme legcons:Item .

C2024A00059:45 a legcons:Subdivision,
        owl:Class,
        dcat:Resource ;
    rdfs:label "Subdivision - S45 Subdivision DSpending requirements for statutory recipient bodies"@en-AU ;
    dct:isPartOf C2024A00059:15 ;
    dct:isReferencedBy C2024A00059: ;
    rdfs:comment "Subdivision DSpending requirements for statutory recipient bodies - Abrievated Graph Key: S45"@en-AU ;
    skos:definition "Subdivision DSpending requirements for statutory recipient bodies"@en-AU ;
    skos:narrower C2024A00059:15 ;
    skos:prefLabel "Subdivision S45"@en-AU ;
    dcat:accessURL <https://www.legislation.gov.au/C2024A00059/asmade/2024-07-09/text/original/epub/OEBPS/document_1/document_1.html#_Toc171508600> ;
    dcat:landingPage "https://www.legislation.gov.au/C2024A00059/asmade/2024-07-09/text/original/epub/OEBPS/document_1/document_1.html#_Toc171508600"^^xsd:anyURI ;
    dcat:theme legcons:Subdivision .

C2024A00059:46 a legcons:Item,
        owl:Class,
        dcat:Resource ;
    rdfs:label "Item - I46 34  Spending of matching paymentsstatutory recipient bodies except the Fisheries Research and Development Corporation"@en-AU ;
    dct:isPartOf C2024A00059:15 ;
    dct:isReferencedBy C2024A00059: ;
    rdfs:comment "34  Spending of matching paymentsstatutory recipient bodies except the Fisheries Research and Development Corporation - Abrievated Graph Key: I46"@en-AU ;
    skos:definition "34  Spending of matching paymentsstatutory recipient bodies except the Fisheries Research and Development Corporation"@en-AU ;
    skos:narrower C2024A00059:15 ;
    skos:prefLabel "Item I46"@en-AU ;
    dcat:accessURL <https://www.legislation.gov.au/C2024A00059/asmade/2024-07-09/text/original/epub/OEBPS/document_1/document_1.html#_Toc171508601> ;
    dcat:landingPage "https://www.legislation.gov.au/C2024A00059/asmade/2024-07-09/text/original/epub/OEBPS/document_1/document_1.html#_Toc171508601"^^xsd:anyURI ;
    dcat:theme legcons:Item .

C2024A00059:47 a legcons:Item,
        owl:Class,
        dcat:Resource ;
    rdfs:label "Item - I47 35  Spending of matching paymentsFisheries Research and Development Corporation"@en-AU ;
    dct:isPartOf C2024A00059:15 ;
    dct:isReferencedBy C2024A00059: ;
    rdfs:comment "35  Spending of matching paymentsFisheries Research and Development Corporation - Abrievated Graph Key: I47"@en-AU ;
    skos:definition "35  Spending of matching paymentsFisheries Research and Development Corporation"@en-AU ;
    skos:narrower C2024A00059:15 ;
    skos:prefLabel "Item I47"@en-AU ;
    dcat:accessURL <https://www.legislation.gov.au/C2024A00059/asmade/2024-07-09/text/original/epub/OEBPS/document_1/document_1.html#_Toc171508602> ;
    dcat:landingPage "https://www.legislation.gov.au/C2024A00059/asmade/2024-07-09/text/original/epub/OEBPS/document_1/document_1.html#_Toc171508602"^^xsd:anyURI ;
    dcat:theme legcons:Item .

C2024A00059:48 a legcons:Division,
        owl:Class,
        dcat:Resource ;
    rdfs:label "Division - D48 Division 4 Other payments to the Fisheries Research and Development Corporation"@en-AU ;
    dct:isPartOf C2024A00059:15 ;
    dct:isReferencedBy C2024A00059: ;
    rdfs:comment "Division 4 Other payments to the Fisheries Research and Development Corporation - Abrievated Graph Key: D48"@en-AU ;
    skos:definition "Division 4 Other payments to the Fisheries Research and Development Corporation"@en-AU ;
    skos:narrower C2024A00059:15 ;
    skos:prefLabel "Division D48"@en-AU ;
    dcat:accessURL <https://www.legislation.gov.au/C2024A00059/asmade/2024-07-09/text/original/epub/OEBPS/document_1/document_1.html#_Toc171508603> ;
    dcat:landingPage "https://www.legislation.gov.au/C2024A00059/asmade/2024-07-09/text/original/epub/OEBPS/document_1/document_1.html#_Toc171508603"^^xsd:anyURI ;
    dcat:theme legcons:Division .

C2024A00059:49 a legcons:Item,
        owl:Class,
        dcat:Resource ;
    rdfs:label "Item - I49 36  Commonwealth to make other payments to the Fisheries Research and Development Corporation"@en-AU ;
    dct:isPartOf C2024A00059:15 ;
    dct:isReferencedBy C2024A00059: ;
    rdfs:comment "36  Commonwealth to make other payments to the Fisheries Research and Development Corporation - Abrievated Graph Key: I49"@en-AU ;
    skos:definition "36  Commonwealth to make other payments to the Fisheries Research and Development Corporation"@en-AU ;
    skos:narrower C2024A00059:15 ;
    skos:prefLabel "Item I49"@en-AU ;
    dcat:accessURL <https://www.legislation.gov.au/C2024A00059/asmade/2024-07-09/text/original/epub/OEBPS/document_1/document_1.html#_Toc171508604> ;
    dcat:landingPage "https://www.legislation.gov.au/C2024A00059/asmade/2024-07-09/text/original/epub/OEBPS/document_1/document_1.html#_Toc171508604"^^xsd:anyURI ;
    dcat:theme legcons:Item .

C2024A00059:5 a legcons:Item,
        owl:Class,
        dcat:Resource ;
    rdfs:label "Item - I5 4  General definitions"@en-AU ;
    dct:isPartOf C2024A00059:1 ;
    dct:isReferencedBy C2024A00059: ;
    rdfs:comment "4  General definitions - Abrievated Graph Key: I5"@en-AU ;
    skos:definition "4  General definitions"@en-AU ;
    skos:narrower C2024A00059:1 ;
    skos:prefLabel "Item I5"@en-AU ;
    dcat:accessURL <https://www.legislation.gov.au/C2024A00059/asmade/2024-07-09/text/original/epub/OEBPS/document_1/document_1.html#_Toc171508560> ;
    dcat:landingPage "https://www.legislation.gov.au/C2024A00059/asmade/2024-07-09/text/original/epub/OEBPS/document_1/document_1.html#_Toc171508560"^^xsd:anyURI ;
    dcat:theme legcons:Item .

C2024A00059:50 a legcons:Division,
        owl:Class,
        dcat:Resource ;
    rdfs:label "Division - D50 Division 5 Appropriation"@en-AU ;
    dct:isPartOf C2024A00059:15 ;
    dct:isReferencedBy C2024A00059: ;
    rdfs:comment "Division 5 Appropriation - Abrievated Graph Key: D50"@en-AU ;
    skos:definition "Division 5 Appropriation"@en-AU ;
    skos:narrower C2024A00059:15 ;
    skos:prefLabel "Division D50"@en-AU ;
    dcat:accessURL <https://www.legislation.gov.au/C2024A00059/asmade/2024-07-09/text/original/epub/OEBPS/document_1/document_1.html#_Toc171508605> ;
    dcat:landingPage "https://www.legislation.gov.au/C2024A00059/asmade/2024-07-09/text/original/epub/OEBPS/document_1/document_1.html#_Toc171508605"^^xsd:anyURI ;
    dcat:theme legcons:Division .

C2024A00059:51 a legcons:Item,
        owl:Class,
        dcat:Resource ;
    rdfs:label "Item - I51 37  Appropriation"@en-AU ;
    dct:isPartOf C2024A00059:15 ;
    dct:isReferencedBy C2024A00059: ;
    rdfs:comment "37  Appropriation - Abrievated Graph Key: I51"@en-AU ;
    skos:definition "37  Appropriation"@en-AU ;
    skos:narrower C2024A00059:15 ;
    skos:prefLabel "Item I51"@en-AU ;
    dcat:accessURL <https://www.legislation.gov.au/C2024A00059/asmade/2024-07-09/text/original/epub/OEBPS/document_1/document_1.html#_Toc171508606> ;
    dcat:landingPage "https://www.legislation.gov.au/C2024A00059/asmade/2024-07-09/text/original/epub/OEBPS/document_1/document_1.html#_Toc171508606"^^xsd:anyURI ;
    dcat:theme legcons:Item .

C2024A00059:52 a legcons:Division,
        owl:Class,
        dcat:Resource ;
    rdfs:label "Division - D52 Division 6 Funding agreements and recipient bodies"@en-AU ;
    dct:isPartOf C2024A00059:15 ;
    dct:isReferencedBy C2024A00059: ;
    rdfs:comment "Division 6 Funding agreements and recipient bodies - Abrievated Graph Key: D52"@en-AU ;
    skos:definition "Division 6 Funding agreements and recipient bodies"@en-AU ;
    skos:narrower C2024A00059:15 ;
    skos:prefLabel "Division D52"@en-AU ;
    dcat:accessURL <https://www.legislation.gov.au/C2024A00059/asmade/2024-07-09/text/original/epub/OEBPS/document_1/document_1.html#_Toc171508607> ;
    dcat:landingPage "https://www.legislation.gov.au/C2024A00059/asmade/2024-07-09/text/original/epub/OEBPS/document_1/document_1.html#_Toc171508607"^^xsd:anyURI ;
    dcat:theme legcons:Division .

C2024A00059:53 a legcons:Subdivision,
        owl:Class,
        dcat:Resource ;
    rdfs:label "Subdivision - S53 Subdivision AFunding agreements and declared recipient bodies"@en-AU ;
    dct:isPartOf C2024A00059:15 ;
    dct:isReferencedBy C2024A00059: ;
    rdfs:comment "Subdivision AFunding agreements and declared recipient bodies - Abrievated Graph Key: S53"@en-AU ;
    skos:definition "Subdivision AFunding agreements and declared recipient bodies"@en-AU ;
    skos:narrower C2024A00059:15 ;
    skos:prefLabel "Subdivision S53"@en-AU ;
    dcat:accessURL <https://www.legislation.gov.au/C2024A00059/asmade/2024-07-09/text/original/epub/OEBPS/document_1/document_1.html#_Toc171508608> ;
    dcat:landingPage "https://www.legislation.gov.au/C2024A00059/asmade/2024-07-09/text/original/epub/OEBPS/document_1/document_1.html#_Toc171508608"^^xsd:anyURI ;
    dcat:theme legcons:Subdivision .

C2024A00059:54 a legcons:Item,
        owl:Class,
        dcat:Resource ;
    rdfs:label "Item - I54 38  Funding agreements with companies"@en-AU ;
    dct:isPartOf C2024A00059:15 ;
    dct:isReferencedBy C2024A00059: ;
    rdfs:comment "38  Funding agreements with companies - Abrievated Graph Key: I54"@en-AU ;
    skos:definition "38  Funding agreements with companies"@en-AU ;
    skos:narrower C2024A00059:15 ;
    skos:prefLabel "Item I54"@en-AU ;
    dcat:accessURL <https://www.legislation.gov.au/C2024A00059/asmade/2024-07-09/text/original/epub/OEBPS/document_1/document_1.html#_Toc171508609> ;
    dcat:landingPage "https://www.legislation.gov.au/C2024A00059/asmade/2024-07-09/text/original/epub/OEBPS/document_1/document_1.html#_Toc171508609"^^xsd:anyURI ;
    dcat:theme legcons:Item .

C2024A00059:55 a legcons:Item,
        owl:Class,
        dcat:Resource ;
    rdfs:label "Item - I55 39  Minister may declare bodies to be recipient bodies"@en-AU ;
    dct:isPartOf C2024A00059:15 ;
    dct:isReferencedBy C2024A00059: ;
    rdfs:comment "39  Minister may declare bodies to be recipient bodies - Abrievated Graph Key: I55"@en-AU ;
    skos:definition "39  Minister may declare bodies to be recipient bodies"@en-AU ;
    skos:narrower C2024A00059:15 ;
    skos:prefLabel "Item I55"@en-AU ;
    dcat:accessURL <https://www.legislation.gov.au/C2024A00059/asmade/2024-07-09/text/original/epub/OEBPS/document_1/document_1.html#_Toc171508610> ;
    dcat:landingPage "https://www.legislation.gov.au/C2024A00059/asmade/2024-07-09/text/original/epub/OEBPS/document_1/document_1.html#_Toc171508610"^^xsd:anyURI ;
    dcat:theme legcons:Item .

C2024A00059:56 a legcons:Item,
        owl:Class,
        dcat:Resource ;
    rdfs:label "Item - I56 40  Minister may revoke declaration of a body as a recipient body"@en-AU ;
    dct:isPartOf C2024A00059:15 ;
    dct:isReferencedBy C2024A00059: ;
    rdfs:comment "40  Minister may revoke declaration of a body as a recipient body - Abrievated Graph Key: I56"@en-AU ;
    skos:definition "40  Minister may revoke declaration of a body as a recipient body"@en-AU ;
    skos:narrower C2024A00059:15 ;
    skos:prefLabel "Item I56"@en-AU ;
    dcat:accessURL <https://www.legislation.gov.au/C2024A00059/asmade/2024-07-09/text/original/epub/OEBPS/document_1/document_1.html#_Toc171508611> ;
    dcat:landingPage "https://www.legislation.gov.au/C2024A00059/asmade/2024-07-09/text/original/epub/OEBPS/document_1/document_1.html#_Toc171508611"^^xsd:anyURI ;
    dcat:theme legcons:Item .

C2024A00059:57 a legcons:Item,
        owl:Class,
        dcat:Resource ;
    rdfs:label "Item - I57 41  Minister may give directions to declared recipient bodies"@en-AU ;
    dct:isPartOf C2024A00059:15 ;
    dct:isReferencedBy C2024A00059: ;
    rdfs:comment "41  Minister may give directions to declared recipient bodies - Abrievated Graph Key: I57"@en-AU ;
    skos:definition "41  Minister may give directions to declared recipient bodies"@en-AU ;
    skos:narrower C2024A00059:15 ;
    skos:prefLabel "Item I57"@en-AU ;
    dcat:accessURL <https://www.legislation.gov.au/C2024A00059/asmade/2024-07-09/text/original/epub/OEBPS/document_1/document_1.html#_Toc171508612> ;
    dcat:landingPage "https://www.legislation.gov.au/C2024A00059/asmade/2024-07-09/text/original/epub/OEBPS/document_1/document_1.html#_Toc171508612"^^xsd:anyURI ;
    dcat:theme legcons:Item .

C2024A00059:58 a legcons:Subdivision,
        owl:Class,
        dcat:Resource ;
    rdfs:label "Subdivision - S58 Subdivision BFunding agreements with statutory recipient bodies"@en-AU ;
    dct:isPartOf C2024A00059:15 ;
    dct:isReferencedBy C2024A00059: ;
    rdfs:comment "Subdivision BFunding agreements with statutory recipient bodies - Abrievated Graph Key: S58"@en-AU ;
    skos:definition "Subdivision BFunding agreements with statutory recipient bodies"@en-AU ;
    skos:narrower C2024A00059:15 ;
    skos:prefLabel "Subdivision S58"@en-AU ;
    dcat:accessURL <https://www.legislation.gov.au/C2024A00059/asmade/2024-07-09/text/original/epub/OEBPS/document_1/document_1.html#_Toc171508613> ;
    dcat:landingPage "https://www.legislation.gov.au/C2024A00059/asmade/2024-07-09/text/original/epub/OEBPS/document_1/document_1.html#_Toc171508613"^^xsd:anyURI ;
    dcat:theme legcons:Subdivision .

C2024A00059:59 a legcons:Item,
        owl:Class,
        dcat:Resource ;
    rdfs:label "Item - I59 42  Funding agreements with statutory recipient bodies"@en-AU ;
    dct:isPartOf C2024A00059:15 ;
    dct:isReferencedBy C2024A00059: ;
    rdfs:comment "42  Funding agreements with statutory recipient bodies - Abrievated Graph Key: I59"@en-AU ;
    skos:definition "42  Funding agreements with statutory recipient bodies"@en-AU ;
    skos:narrower C2024A00059:15 ;
    skos:prefLabel "Item I59"@en-AU ;
    dcat:accessURL <https://www.legislation.gov.au/C2024A00059/asmade/2024-07-09/text/original/epub/OEBPS/document_1/document_1.html#_Toc171508614> ;
    dcat:landingPage "https://www.legislation.gov.au/C2024A00059/asmade/2024-07-09/text/original/epub/OEBPS/document_1/document_1.html#_Toc171508614"^^xsd:anyURI ;
    dcat:theme legcons:Item .

C2024A00059:6 a legcons:Item,
        owl:Class,
        dcat:Resource ;
    rdfs:label "Item - I6 5  Declared fishery"@en-AU ;
    dct:isPartOf C2024A00059:1 ;
    dct:isReferencedBy C2024A00059: ;
    rdfs:comment "5  Declared fishery - Abrievated Graph Key: I6"@en-AU ;
    skos:definition "5  Declared fishery"@en-AU ;
    skos:narrower C2024A00059:1 ;
    skos:prefLabel "Item I6"@en-AU ;
    dcat:accessURL <https://www.legislation.gov.au/C2024A00059/asmade/2024-07-09/text/original/epub/OEBPS/document_1/document_1.html#_Toc171508561> ;
    dcat:landingPage "https://www.legislation.gov.au/C2024A00059/asmade/2024-07-09/text/original/epub/OEBPS/document_1/document_1.html#_Toc171508561"^^xsd:anyURI ;
    dcat:theme legcons:Item .

C2024A00059:62 a legcons:Item,
        owl:Class,
        dcat:Resource ;
    rdfs:label "Item - I62 43  Simplified outline of this Part"@en-AU ;
    dct:isPartOf C2024A00059:61 ;
    dct:isReferencedBy C2024A00059: ;
    rdfs:comment "43  Simplified outline of this Part - Abrievated Graph Key: I62"@en-AU ;
    skos:definition "43  Simplified outline of this Part"@en-AU ;
    skos:narrower C2024A00059:61 ;
    skos:prefLabel "Item I62"@en-AU ;
    dcat:accessURL <https://www.legislation.gov.au/C2024A00059/asmade/2024-07-09/text/original/epub/OEBPS/document_1/document_1.html#_Toc171508617> ;
    dcat:landingPage "https://www.legislation.gov.au/C2024A00059/asmade/2024-07-09/text/original/epub/OEBPS/document_1/document_1.html#_Toc171508617"^^xsd:anyURI ;
    dcat:theme legcons:Item .

C2024A00059:65 a legcons:Item,
        owl:Class,
        dcat:Resource ;
    rdfs:label "Item - I65 44  Commonwealth to make paymentscollected amounts relating to biosecurity activity"@en-AU ;
    dct:isPartOf C2024A00059:64 ;
    dct:isReferencedBy C2024A00059: ;
    rdfs:comment "44  Commonwealth to make paymentscollected amounts relating to biosecurity activity - Abrievated Graph Key: I65"@en-AU ;
    skos:definition "44  Commonwealth to make paymentscollected amounts relating to biosecurity activity"@en-AU ;
    skos:narrower C2024A00059:64 ;
    skos:prefLabel "Item I65"@en-AU ;
    dcat:accessURL <https://www.legislation.gov.au/C2024A00059/asmade/2024-07-09/text/original/epub/OEBPS/document_1/document_1.html#_Toc171508620> ;
    dcat:landingPage "https://www.legislation.gov.au/C2024A00059/asmade/2024-07-09/text/original/epub/OEBPS/document_1/document_1.html#_Toc171508620"^^xsd:anyURI ;
    dcat:theme legcons:Item .

C2024A00059:66 a legcons:Item,
        owl:Class,
        dcat:Resource ;
    rdfs:label "Item - I66 45  Application of money"@en-AU ;
    dct:isPartOf C2024A00059:64 ;
    dct:isReferencedBy C2024A00059: ;
    rdfs:comment "45  Application of money - Abrievated Graph Key: I66"@en-AU ;
    skos:definition "45  Application of money"@en-AU ;
    skos:narrower C2024A00059:64 ;
    skos:prefLabel "Item I66"@en-AU ;
    dcat:accessURL <https://www.legislation.gov.au/C2024A00059/asmade/2024-07-09/text/original/epub/OEBPS/document_1/document_1.html#_Toc171508621> ;
    dcat:landingPage "https://www.legislation.gov.au/C2024A00059/asmade/2024-07-09/text/original/epub/OEBPS/document_1/document_1.html#_Toc171508621"^^xsd:anyURI ;
    dcat:theme legcons:Item .

C2024A00059:67 a legcons:Item,
        owl:Class,
        dcat:Resource ;
    rdfs:label "Item - I67 46  Effect of refunds"@en-AU ;
    dct:isPartOf C2024A00059:64 ;
    dct:isReferencedBy C2024A00059: ;
    rdfs:comment "46  Effect of refunds - Abrievated Graph Key: I67"@en-AU ;
    skos:definition "46  Effect of refunds"@en-AU ;
    skos:narrower C2024A00059:64 ;
    skos:prefLabel "Item I67"@en-AU ;
    dcat:accessURL <https://www.legislation.gov.au/C2024A00059/asmade/2024-07-09/text/original/epub/OEBPS/document_1/document_1.html#_Toc171508622> ;
    dcat:landingPage "https://www.legislation.gov.au/C2024A00059/asmade/2024-07-09/text/original/epub/OEBPS/document_1/document_1.html#_Toc171508622"^^xsd:anyURI ;
    dcat:theme legcons:Item .

C2024A00059:68 a legcons:Item,
        owl:Class,
        dcat:Resource ;
    rdfs:label "Item - I68 47  Recoverable paymentspayment of debt"@en-AU ;
    dct:isPartOf C2024A00059:64 ;
    dct:isReferencedBy C2024A00059: ;
    rdfs:comment "47  Recoverable paymentspayment of debt - Abrievated Graph Key: I68"@en-AU ;
    skos:definition "47  Recoverable paymentspayment of debt"@en-AU ;
    skos:narrower C2024A00059:64 ;
    skos:prefLabel "Item I68"@en-AU ;
    dcat:accessURL <https://www.legislation.gov.au/C2024A00059/asmade/2024-07-09/text/original/epub/OEBPS/document_1/document_1.html#_Toc171508623> ;
    dcat:landingPage "https://www.legislation.gov.au/C2024A00059/asmade/2024-07-09/text/original/epub/OEBPS/document_1/document_1.html#_Toc171508623"^^xsd:anyURI ;
    dcat:theme legcons:Item .

C2024A00059:7 a legcons:Item,
        owl:Class,
        dcat:Resource ;
    rdfs:label "Item - I7 6  Designated primary industry sectors for declared recipient bodies"@en-AU ;
    dct:isPartOf C2024A00059:1 ;
    dct:isReferencedBy C2024A00059: ;
    rdfs:comment "6  Designated primary industry sectors for declared recipient bodies - Abrievated Graph Key: I7"@en-AU ;
    skos:definition "6  Designated primary industry sectors for declared recipient bodies"@en-AU ;
    skos:narrower C2024A00059:1 ;
    skos:prefLabel "Item I7"@en-AU ;
    dcat:accessURL <https://www.legislation.gov.au/C2024A00059/asmade/2024-07-09/text/original/epub/OEBPS/document_1/document_1.html#_Toc171508562> ;
    dcat:landingPage "https://www.legislation.gov.au/C2024A00059/asmade/2024-07-09/text/original/epub/OEBPS/document_1/document_1.html#_Toc171508562"^^xsd:anyURI ;
    dcat:theme legcons:Item .

C2024A00059:70 a legcons:Item,
        owl:Class,
        dcat:Resource ;
    rdfs:label "Item - I70 48  Commonwealth to make paymentscollected amounts relating to biosecurity response"@en-AU ;
    dct:isPartOf C2024A00059:69 ;
    dct:isReferencedBy C2024A00059: ;
    rdfs:comment "48  Commonwealth to make paymentscollected amounts relating to biosecurity response - Abrievated Graph Key: I70"@en-AU ;
    skos:definition "48  Commonwealth to make paymentscollected amounts relating to biosecurity response"@en-AU ;
    skos:narrower C2024A00059:69 ;
    skos:prefLabel "Item I70"@en-AU ;
    dcat:accessURL <https://www.legislation.gov.au/C2024A00059/asmade/2024-07-09/text/original/epub/OEBPS/document_1/document_1.html#_Toc171508625> ;
    dcat:landingPage "https://www.legislation.gov.au/C2024A00059/asmade/2024-07-09/text/original/epub/OEBPS/document_1/document_1.html#_Toc171508625"^^xsd:anyURI ;
    dcat:theme legcons:Item .

C2024A00059:71 a legcons:Item,
        owl:Class,
        dcat:Resource ;
    rdfs:label "Item - I71 49  Application of money"@en-AU ;
    dct:isPartOf C2024A00059:69 ;
    dct:isReferencedBy C2024A00059: ;
    rdfs:comment "49  Application of money - Abrievated Graph Key: I71"@en-AU ;
    skos:definition "49  Application of money"@en-AU ;
    skos:narrower C2024A00059:69 ;
    skos:prefLabel "Item I71"@en-AU ;
    dcat:accessURL <https://www.legislation.gov.au/C2024A00059/asmade/2024-07-09/text/original/epub/OEBPS/document_1/document_1.html#_Toc171508626> ;
    dcat:landingPage "https://www.legislation.gov.au/C2024A00059/asmade/2024-07-09/text/original/epub/OEBPS/document_1/document_1.html#_Toc171508626"^^xsd:anyURI ;
    dcat:theme legcons:Item .

C2024A00059:72 a legcons:Item,
        owl:Class,
        dcat:Resource ;
    rdfs:label "Item - I72 50  Effect of refunds"@en-AU ;
    dct:isPartOf C2024A00059:69 ;
    dct:isReferencedBy C2024A00059: ;
    rdfs:comment "50  Effect of refunds - Abrievated Graph Key: I72"@en-AU ;
    skos:definition "50  Effect of refunds"@en-AU ;
    skos:narrower C2024A00059:69 ;
    skos:prefLabel "Item I72"@en-AU ;
    dcat:accessURL <https://www.legislation.gov.au/C2024A00059/asmade/2024-07-09/text/original/epub/OEBPS/document_1/document_1.html#_Toc171508627> ;
    dcat:landingPage "https://www.legislation.gov.au/C2024A00059/asmade/2024-07-09/text/original/epub/OEBPS/document_1/document_1.html#_Toc171508627"^^xsd:anyURI ;
    dcat:theme legcons:Item .

C2024A00059:73 a legcons:Item,
        owl:Class,
        dcat:Resource ;
    rdfs:label "Item - I73 51  Recoverable paymentspayment of debt"@en-AU ;
    dct:isPartOf C2024A00059:69 ;
    dct:isReferencedBy C2024A00059: ;
    rdfs:comment "51  Recoverable paymentspayment of debt - Abrievated Graph Key: I73"@en-AU ;
    skos:definition "51  Recoverable paymentspayment of debt"@en-AU ;
    skos:narrower C2024A00059:69 ;
    skos:prefLabel "Item I73"@en-AU ;
    dcat:accessURL <https://www.legislation.gov.au/C2024A00059/asmade/2024-07-09/text/original/epub/OEBPS/document_1/document_1.html#_Toc171508628> ;
    dcat:landingPage "https://www.legislation.gov.au/C2024A00059/asmade/2024-07-09/text/original/epub/OEBPS/document_1/document_1.html#_Toc171508628"^^xsd:anyURI ;
    dcat:theme legcons:Item .

C2024A00059:75 a legcons:Item,
        owl:Class,
        dcat:Resource ;
    rdfs:label "Item - I75 52  Appropriation"@en-AU ;
    dct:isPartOf C2024A00059:74 ;
    dct:isReferencedBy C2024A00059: ;
    rdfs:comment "52  Appropriation - Abrievated Graph Key: I75"@en-AU ;
    skos:definition "52  Appropriation"@en-AU ;
    skos:narrower C2024A00059:74 ;
    skos:prefLabel "Item I75"@en-AU ;
    dcat:accessURL <https://www.legislation.gov.au/C2024A00059/asmade/2024-07-09/text/original/epub/OEBPS/document_1/document_1.html#_Toc171508630> ;
    dcat:landingPage "https://www.legislation.gov.au/C2024A00059/asmade/2024-07-09/text/original/epub/OEBPS/document_1/document_1.html#_Toc171508630"^^xsd:anyURI ;
    dcat:theme legcons:Item .

C2024A00059:78 a legcons:Item,
        owl:Class,
        dcat:Resource ;
    rdfs:label "Item - I78 53  Simplified outline of this Part"@en-AU ;
    dct:isPartOf C2024A00059:77 ;
    dct:isReferencedBy C2024A00059: ;
    rdfs:comment "53  Simplified outline of this Part - Abrievated Graph Key: I78"@en-AU ;
    skos:definition "53  Simplified outline of this Part"@en-AU ;
    skos:narrower C2024A00059:77 ;
    skos:prefLabel "Item I78"@en-AU ;
    dcat:accessURL <https://www.legislation.gov.au/C2024A00059/asmade/2024-07-09/text/original/epub/OEBPS/document_1/document_1.html#_Toc171508633> ;
    dcat:landingPage "https://www.legislation.gov.au/C2024A00059/asmade/2024-07-09/text/original/epub/OEBPS/document_1/document_1.html#_Toc171508633"^^xsd:anyURI ;
    dcat:theme legcons:Item .

C2024A00059:8 a legcons:Item,
        owl:Class,
        dcat:Resource ;
    rdfs:label "Item - I8 7  Definition of relevant animal health body"@en-AU ;
    dct:isPartOf C2024A00059:1 ;
    dct:isReferencedBy C2024A00059: ;
    rdfs:comment "7  Definition of relevant animal health body - Abrievated Graph Key: I8"@en-AU ;
    skos:definition "7  Definition of relevant animal health body"@en-AU ;
    skos:narrower C2024A00059:1 ;
    skos:prefLabel "Item I8"@en-AU ;
    dcat:accessURL <https://www.legislation.gov.au/C2024A00059/asmade/2024-07-09/text/original/epub/OEBPS/document_1/document_1.html#_Toc171508563> ;
    dcat:landingPage "https://www.legislation.gov.au/C2024A00059/asmade/2024-07-09/text/original/epub/OEBPS/document_1/document_1.html#_Toc171508563"^^xsd:anyURI ;
    dcat:theme legcons:Item .

C2024A00059:81 a legcons:Item,
        owl:Class,
        dcat:Resource ;
    rdfs:label "Item - I81 54  Commonwealth to make paymentscollected amounts relating to biosecurity activity"@en-AU ;
    dct:isPartOf C2024A00059:80 ;
    dct:isReferencedBy C2024A00059: ;
    rdfs:comment "54  Commonwealth to make paymentscollected amounts relating to biosecurity activity - Abrievated Graph Key: I81"@en-AU ;
    skos:definition "54  Commonwealth to make paymentscollected amounts relating to biosecurity activity"@en-AU ;
    skos:narrower C2024A00059:80 ;
    skos:prefLabel "Item I81"@en-AU ;
    dcat:accessURL <https://www.legislation.gov.au/C2024A00059/asmade/2024-07-09/text/original/epub/OEBPS/document_1/document_1.html#_Toc171508636> ;
    dcat:landingPage "https://www.legislation.gov.au/C2024A00059/asmade/2024-07-09/text/original/epub/OEBPS/document_1/document_1.html#_Toc171508636"^^xsd:anyURI ;
    dcat:theme legcons:Item .

C2024A00059:82 a legcons:Item,
        owl:Class,
        dcat:Resource ;
    rdfs:label "Item - I82 55  Application of money"@en-AU ;
    dct:isPartOf C2024A00059:80 ;
    dct:isReferencedBy C2024A00059: ;
    rdfs:comment "55  Application of money - Abrievated Graph Key: I82"@en-AU ;
    skos:definition "55  Application of money"@en-AU ;
    skos:narrower C2024A00059:80 ;
    skos:prefLabel "Item I82"@en-AU ;
    dcat:accessURL <https://www.legislation.gov.au/C2024A00059/asmade/2024-07-09/text/original/epub/OEBPS/document_1/document_1.html#_Toc171508637> ;
    dcat:landingPage "https://www.legislation.gov.au/C2024A00059/asmade/2024-07-09/text/original/epub/OEBPS/document_1/document_1.html#_Toc171508637"^^xsd:anyURI ;
    dcat:theme legcons:Item .

C2024A00059:83 a legcons:Item,
        owl:Class,
        dcat:Resource ;
    rdfs:label "Item - I83 56  Effect of refunds"@en-AU ;
    dct:isPartOf C2024A00059:80 ;
    dct:isReferencedBy C2024A00059: ;
    rdfs:comment "56  Effect of refunds - Abrievated Graph Key: I83"@en-AU ;
    skos:definition "56  Effect of refunds"@en-AU ;
    skos:narrower C2024A00059:80 ;
    skos:prefLabel "Item I83"@en-AU ;
    dcat:accessURL <https://www.legislation.gov.au/C2024A00059/asmade/2024-07-09/text/original/epub/OEBPS/document_1/document_1.html#_Toc171508638> ;
    dcat:landingPage "https://www.legislation.gov.au/C2024A00059/asmade/2024-07-09/text/original/epub/OEBPS/document_1/document_1.html#_Toc171508638"^^xsd:anyURI ;
    dcat:theme legcons:Item .

C2024A00059:84 a legcons:Item,
        owl:Class,
        dcat:Resource ;
    rdfs:label "Item - I84 57  Recoverable paymentspayment of debt"@en-AU ;
    dct:isPartOf C2024A00059:80 ;
    dct:isReferencedBy C2024A00059: ;
    rdfs:comment "57  Recoverable paymentspayment of debt - Abrievated Graph Key: I84"@en-AU ;
    skos:definition "57  Recoverable paymentspayment of debt"@en-AU ;
    skos:narrower C2024A00059:80 ;
    skos:prefLabel "Item I84"@en-AU ;
    dcat:accessURL <https://www.legislation.gov.au/C2024A00059/asmade/2024-07-09/text/original/epub/OEBPS/document_1/document_1.html#_Toc171508639> ;
    dcat:landingPage "https://www.legislation.gov.au/C2024A00059/asmade/2024-07-09/text/original/epub/OEBPS/document_1/document_1.html#_Toc171508639"^^xsd:anyURI ;
    dcat:theme legcons:Item .

C2024A00059:86 a legcons:Item,
        owl:Class,
        dcat:Resource ;
    rdfs:label "Item - I86 58  Commonwealth to make paymentscollected amounts relating to biosecurity response"@en-AU ;
    dct:isPartOf C2024A00059:85 ;
    dct:isReferencedBy C2024A00059: ;
    rdfs:comment "58  Commonwealth to make paymentscollected amounts relating to biosecurity response - Abrievated Graph Key: I86"@en-AU ;
    skos:definition "58  Commonwealth to make paymentscollected amounts relating to biosecurity response"@en-AU ;
    skos:narrower C2024A00059:85 ;
    skos:prefLabel "Item I86"@en-AU ;
    dcat:accessURL <https://www.legislation.gov.au/C2024A00059/asmade/2024-07-09/text/original/epub/OEBPS/document_1/document_1.html#_Toc171508641> ;
    dcat:landingPage "https://www.legislation.gov.au/C2024A00059/asmade/2024-07-09/text/original/epub/OEBPS/document_1/document_1.html#_Toc171508641"^^xsd:anyURI ;
    dcat:theme legcons:Item .

C2024A00059:87 a legcons:Item,
        owl:Class,
        dcat:Resource ;
    rdfs:label "Item - I87 59  Application of money"@en-AU ;
    dct:isPartOf C2024A00059:85 ;
    dct:isReferencedBy C2024A00059: ;
    rdfs:comment "59  Application of money - Abrievated Graph Key: I87"@en-AU ;
    skos:definition "59  Application of money"@en-AU ;
    skos:narrower C2024A00059:85 ;
    skos:prefLabel "Item I87"@en-AU ;
    dcat:accessURL <https://www.legislation.gov.au/C2024A00059/asmade/2024-07-09/text/original/epub/OEBPS/document_1/document_1.html#_Toc171508642> ;
    dcat:landingPage "https://www.legislation.gov.au/C2024A00059/asmade/2024-07-09/text/original/epub/OEBPS/document_1/document_1.html#_Toc171508642"^^xsd:anyURI ;
    dcat:theme legcons:Item .

C2024A00059:88 a legcons:Item,
        owl:Class,
        dcat:Resource ;
    rdfs:label "Item - I88 60  Effect of refunds"@en-AU ;
    dct:isPartOf C2024A00059:85 ;
    dct:isReferencedBy C2024A00059: ;
    rdfs:comment "60  Effect of refunds - Abrievated Graph Key: I88"@en-AU ;
    skos:definition "60  Effect of refunds"@en-AU ;
    skos:narrower C2024A00059:85 ;
    skos:prefLabel "Item I88"@en-AU ;
    dcat:accessURL <https://www.legislation.gov.au/C2024A00059/asmade/2024-07-09/text/original/epub/OEBPS/document_1/document_1.html#_Toc171508643> ;
    dcat:landingPage "https://www.legislation.gov.au/C2024A00059/asmade/2024-07-09/text/original/epub/OEBPS/document_1/document_1.html#_Toc171508643"^^xsd:anyURI ;
    dcat:theme legcons:Item .

C2024A00059:89 a legcons:Item,
        owl:Class,
        dcat:Resource ;
    rdfs:label "Item - I89 61  Recoverable paymentspayment of debt"@en-AU ;
    dct:isPartOf C2024A00059:85 ;
    dct:isReferencedBy C2024A00059: ;
    rdfs:comment "61  Recoverable paymentspayment of debt - Abrievated Graph Key: I89"@en-AU ;
    skos:definition "61  Recoverable paymentspayment of debt"@en-AU ;
    skos:narrower C2024A00059:85 ;
    skos:prefLabel "Item I89"@en-AU ;
    dcat:accessURL <https://www.legislation.gov.au/C2024A00059/asmade/2024-07-09/text/original/epub/OEBPS/document_1/document_1.html#_Toc171508644> ;
    dcat:landingPage "https://www.legislation.gov.au/C2024A00059/asmade/2024-07-09/text/original/epub/OEBPS/document_1/document_1.html#_Toc171508644"^^xsd:anyURI ;
    dcat:theme legcons:Item .

C2024A00059:9 a legcons:Item,
        owl:Class,
        dcat:Resource ;
    rdfs:label "Item - I9 8  Definition of relevant plant health body"@en-AU ;
    dct:isPartOf C2024A00059:1 ;
    dct:isReferencedBy C2024A00059: ;
    rdfs:comment "8  Definition of relevant plant health body - Abrievated Graph Key: I9"@en-AU ;
    skos:definition "8  Definition of relevant plant health body"@en-AU ;
    skos:narrower C2024A00059:1 ;
    skos:prefLabel "Item I9"@en-AU ;
    dcat:accessURL <https://www.legislation.gov.au/C2024A00059/asmade/2024-07-09/text/original/epub/OEBPS/document_1/document_1.html#_Toc171508564> ;
    dcat:landingPage "https://www.legislation.gov.au/C2024A00059/asmade/2024-07-09/text/original/epub/OEBPS/document_1/document_1.html#_Toc171508564"^^xsd:anyURI ;
    dcat:theme legcons:Item .

C2024A00059:91 a legcons:Item,
        owl:Class,
        dcat:Resource ;
    rdfs:label "Item - I91 62  Appropriation"@en-AU ;
    dct:isPartOf C2024A00059:90 ;
    dct:isReferencedBy C2024A00059: ;
    rdfs:comment "62  Appropriation - Abrievated Graph Key: I91"@en-AU ;
    skos:definition "62  Appropriation"@en-AU ;
    skos:narrower C2024A00059:90 ;
    skos:prefLabel "Item I91"@en-AU ;
    dcat:accessURL <https://www.legislation.gov.au/C2024A00059/asmade/2024-07-09/text/original/epub/OEBPS/document_1/document_1.html#_Toc171508646> ;
    dcat:landingPage "https://www.legislation.gov.au/C2024A00059/asmade/2024-07-09/text/original/epub/OEBPS/document_1/document_1.html#_Toc171508646"^^xsd:anyURI ;
    dcat:theme legcons:Item .

C2024A00059:94 a legcons:Item,
        owl:Class,
        dcat:Resource ;
    rdfs:label "Item - I94 63  Simplified outline of this Part"@en-AU ;
    dct:isPartOf C2024A00059:93 ;
    dct:isReferencedBy C2024A00059: ;
    rdfs:comment "63  Simplified outline of this Part - Abrievated Graph Key: I94"@en-AU ;
    skos:definition "63  Simplified outline of this Part"@en-AU ;
    skos:narrower C2024A00059:93 ;
    skos:prefLabel "Item I94"@en-AU ;
    dcat:accessURL <https://www.legislation.gov.au/C2024A00059/asmade/2024-07-09/text/original/epub/OEBPS/document_1/document_1.html#_Toc171508649> ;
    dcat:landingPage "https://www.legislation.gov.au/C2024A00059/asmade/2024-07-09/text/original/epub/OEBPS/document_1/document_1.html#_Toc171508649"^^xsd:anyURI ;
    dcat:theme legcons:Item .

C2024A00059:96 a legcons:Item,
        owl:Class,
        dcat:Resource ;
    rdfs:label "Item - I96 64  National Residue Survey Special Account"@en-AU ;
    dct:isPartOf C2024A00059:95 ;
    dct:isReferencedBy C2024A00059: ;
    rdfs:comment "64  National Residue Survey Special Account - Abrievated Graph Key: I96"@en-AU ;
    skos:definition "64  National Residue Survey Special Account"@en-AU ;
    skos:narrower C2024A00059:95 ;
    skos:prefLabel "Item I96"@en-AU ;
    dcat:accessURL <https://www.legislation.gov.au/C2024A00059/asmade/2024-07-09/text/original/epub/OEBPS/document_1/document_1.html#_Toc171508651> ;
    dcat:landingPage "https://www.legislation.gov.au/C2024A00059/asmade/2024-07-09/text/original/epub/OEBPS/document_1/document_1.html#_Toc171508651"^^xsd:anyURI ;
    dcat:theme legcons:Item .

C2024A00059:97 a legcons:Item,
        owl:Class,
        dcat:Resource ;
    rdfs:label "Item - I97 65  Credits to the National Residue Survey Special Account"@en-AU ;
    dct:isPartOf C2024A00059:95 ;
    dct:isReferencedBy C2024A00059: ;
    rdfs:comment "65  Credits to the National Residue Survey Special Account - Abrievated Graph Key: I97"@en-AU ;
    skos:definition "65  Credits to the National Residue Survey Special Account"@en-AU ;
    skos:narrower C2024A00059:95 ;
    skos:prefLabel "Item I97"@en-AU ;
    dcat:accessURL <https://www.legislation.gov.au/C2024A00059/asmade/2024-07-09/text/original/epub/OEBPS/document_1/document_1.html#_Toc171508652> ;
    dcat:landingPage "https://www.legislation.gov.au/C2024A00059/asmade/2024-07-09/text/original/epub/OEBPS/document_1/document_1.html#_Toc171508652"^^xsd:anyURI ;
    dcat:theme legcons:Item .

C2024A00059:98 a legcons:Item,
        owl:Class,
        dcat:Resource ;
    rdfs:label "Item - I98 66  Purposes of the National Residue Survey Special Account"@en-AU ;
    dct:isPartOf C2024A00059:95 ;
    dct:isReferencedBy C2024A00059: ;
    rdfs:comment "66  Purposes of the National Residue Survey Special Account - Abrievated Graph Key: I98"@en-AU ;
    skos:definition "66  Purposes of the National Residue Survey Special Account"@en-AU ;
    skos:narrower C2024A00059:95 ;
    skos:prefLabel "Item I98"@en-AU ;
    dcat:accessURL <https://www.legislation.gov.au/C2024A00059/asmade/2024-07-09/text/original/epub/OEBPS/document_1/document_1.html#_Toc171508653> ;
    dcat:landingPage "https://www.legislation.gov.au/C2024A00059/asmade/2024-07-09/text/original/epub/OEBPS/document_1/document_1.html#_Toc171508653"^^xsd:anyURI ;
    dcat:theme legcons:Item .

C2024A00059:99 a legcons:Item,
        owl:Class,
        dcat:Resource ;
    rdfs:label "Item - I99 67  Report about National Residue Survey Special Account"@en-AU ;
    dct:isPartOf C2024A00059:95 ;
    dct:isReferencedBy C2024A00059: ;
    rdfs:comment "67  Report about National Residue Survey Special Account - Abrievated Graph Key: I99"@en-AU ;
    skos:definition "67  Report about National Residue Survey Special Account"@en-AU ;
    skos:narrower C2024A00059:95 ;
    skos:prefLabel "Item I99"@en-AU ;
    dcat:accessURL <https://www.legislation.gov.au/C2024A00059/asmade/2024-07-09/text/original/epub/OEBPS/document_1/document_1.html#_Toc171508654> ;
    dcat:landingPage "https://www.legislation.gov.au/C2024A00059/asmade/2024-07-09/text/original/epub/OEBPS/document_1/document_1.html#_Toc171508654"^^xsd:anyURI ;
    dcat:theme legcons:Item .

C2024A00059:119 a legcons:Division,
        owl:Class,
        dcat:Resource ;
    rdfs:label "Division - D119 Division 1 Simplified outline of this Part"@en-AU ;
    dct:hasPart C2024A00059:120 ;
    dct:isPartOf C2024A00059:118 ;
    dct:isReferencedBy C2024A00059: ;
    rdfs:comment "Division 1 Simplified outline of this Part - Abrievated Graph Key: D119"@en-AU ;
    skos:broader C2024A00059:120 ;
    skos:definition "Division 1 Simplified outline of this Part"@en-AU ;
    skos:narrower C2024A00059:118 ;
    skos:prefLabel "Division D119"@en-AU ;
    dcat:accessURL <https://www.legislation.gov.au/C2024A00059/asmade/2024-07-09/text/original/epub/OEBPS/document_1/document_1.html#_Toc171508674> ;
    dcat:landingPage "https://www.legislation.gov.au/C2024A00059/asmade/2024-07-09/text/original/epub/OEBPS/document_1/document_1.html#_Toc171508674"^^xsd:anyURI ;
    dcat:theme legcons:Division .

C2024A00059:16 a legcons:Division,
        owl:Class,
        dcat:Resource ;
    rdfs:label "Division - D16 Division 1 Simplified outline of this Part"@en-AU ;
    dct:hasPart C2024A00059:17 ;
    dct:isPartOf C2024A00059:15 ;
    dct:isReferencedBy C2024A00059: ;
    rdfs:comment "Division 1 Simplified outline of this Part - Abrievated Graph Key: D16"@en-AU ;
    skos:broader C2024A00059:17 ;
    skos:definition "Division 1 Simplified outline of this Part"@en-AU ;
    skos:narrower C2024A00059:15 ;
    skos:prefLabel "Division D16"@en-AU ;
    dcat:accessURL <https://www.legislation.gov.au/C2024A00059/asmade/2024-07-09/text/original/epub/OEBPS/document_1/document_1.html#_Toc171508571> ;
    dcat:landingPage "https://www.legislation.gov.au/C2024A00059/asmade/2024-07-09/text/original/epub/OEBPS/document_1/document_1.html#_Toc171508571"^^xsd:anyURI ;
    dcat:theme legcons:Division .

C2024A00059:60 a legcons:Part,
        owl:Class,
        dcat:Resource ;
    rdfs:label "Part - P60 Part 3 Funding for Animal Health Australia"@en-AU ;
    dct:hasPart C2024A00059:61,
        C2024A00059:63 ;
    dct:isReferencedBy C2024A00059: ;
    rdfs:comment "Part 3 Funding for Animal Health Australia - Abrievated Graph Key: P60"@en-AU ;
    skos:broader C2024A00059:61,
        C2024A00059:63 ;
    skos:definition "Part 3 Funding for Animal Health Australia"@en-AU ;
    skos:prefLabel "Part P60"@en-AU ;
    dcat:accessURL <https://www.legislation.gov.au/C2024A00059/asmade/2024-07-09/text/original/epub/OEBPS/document_1/document_1.html#_Toc171508615> ;
    dcat:landingPage "https://www.legislation.gov.au/C2024A00059/asmade/2024-07-09/text/original/epub/OEBPS/document_1/document_1.html#_Toc171508615"^^xsd:anyURI ;
    dcat:theme legcons:Part .

C2024A00059:61 a legcons:Division,
        owl:Class,
        dcat:Resource ;
    rdfs:label "Division - D61 Division 1 Simplified outline of this Part"@en-AU ;
    dct:hasPart C2024A00059:62 ;
    dct:isPartOf C2024A00059:60 ;
    dct:isReferencedBy C2024A00059: ;
    rdfs:comment "Division 1 Simplified outline of this Part - Abrievated Graph Key: D61"@en-AU ;
    skos:broader C2024A00059:62 ;
    skos:definition "Division 1 Simplified outline of this Part"@en-AU ;
    skos:narrower C2024A00059:60 ;
    skos:prefLabel "Division D61"@en-AU ;
    dcat:accessURL <https://www.legislation.gov.au/C2024A00059/asmade/2024-07-09/text/original/epub/OEBPS/document_1/document_1.html#_Toc171508616> ;
    dcat:landingPage "https://www.legislation.gov.au/C2024A00059/asmade/2024-07-09/text/original/epub/OEBPS/document_1/document_1.html#_Toc171508616"^^xsd:anyURI ;
    dcat:theme legcons:Division .

C2024A00059:74 a legcons:Subdivision,
        owl:Class,
        dcat:Resource ;
    rdfs:label "Subdivision - S74 Subdivision CAppropriation"@en-AU ;
    dct:hasPart C2024A00059:75 ;
    dct:isPartOf C2024A00059:63 ;
    dct:isReferencedBy C2024A00059: ;
    rdfs:comment "Subdivision CAppropriation - Abrievated Graph Key: S74"@en-AU ;
    skos:broader C2024A00059:75 ;
    skos:definition "Subdivision CAppropriation"@en-AU ;
    skos:narrower C2024A00059:63 ;
    skos:prefLabel "Subdivision S74"@en-AU ;
    dcat:accessURL <https://www.legislation.gov.au/C2024A00059/asmade/2024-07-09/text/original/epub/OEBPS/document_1/document_1.html#_Toc171508629> ;
    dcat:landingPage "https://www.legislation.gov.au/C2024A00059/asmade/2024-07-09/text/original/epub/OEBPS/document_1/document_1.html#_Toc171508629"^^xsd:anyURI ;
    dcat:theme legcons:Subdivision .

C2024A00059:76 a legcons:Part,
        owl:Class,
        dcat:Resource ;
    rdfs:label "Part - P76 Part 4 Funding for Plant Health Australia"@en-AU ;
    dct:hasPart C2024A00059:77,
        C2024A00059:79 ;
    dct:isReferencedBy C2024A00059: ;
    rdfs:comment "Part 4 Funding for Plant Health Australia - Abrievated Graph Key: P76"@en-AU ;
    skos:broader C2024A00059:77,
        C2024A00059:79 ;
    skos:definition "Part 4 Funding for Plant Health Australia"@en-AU ;
    skos:prefLabel "Part P76"@en-AU ;
    dcat:accessURL <https://www.legislation.gov.au/C2024A00059/asmade/2024-07-09/text/original/epub/OEBPS/document_1/document_1.html#_Toc171508631> ;
    dcat:landingPage "https://www.legislation.gov.au/C2024A00059/asmade/2024-07-09/text/original/epub/OEBPS/document_1/document_1.html#_Toc171508631"^^xsd:anyURI ;
    dcat:theme legcons:Part .

C2024A00059:77 a legcons:Division,
        owl:Class,
        dcat:Resource ;
    rdfs:label "Division - D77 Division 1 Simplified outline of this Part"@en-AU ;
    dct:hasPart C2024A00059:78 ;
    dct:isPartOf C2024A00059:76 ;
    dct:isReferencedBy C2024A00059: ;
    rdfs:comment "Division 1 Simplified outline of this Part - Abrievated Graph Key: D77"@en-AU ;
    skos:broader C2024A00059:78 ;
    skos:definition "Division 1 Simplified outline of this Part"@en-AU ;
    skos:narrower C2024A00059:76 ;
    skos:prefLabel "Division D77"@en-AU ;
    dcat:accessURL <https://www.legislation.gov.au/C2024A00059/asmade/2024-07-09/text/original/epub/OEBPS/document_1/document_1.html#_Toc171508632> ;
    dcat:landingPage "https://www.legislation.gov.au/C2024A00059/asmade/2024-07-09/text/original/epub/OEBPS/document_1/document_1.html#_Toc171508632"^^xsd:anyURI ;
    dcat:theme legcons:Division .

C2024A00059:90 a legcons:Subdivision,
        owl:Class,
        dcat:Resource ;
    rdfs:label "Subdivision - S90 Subdivision CAppropriation"@en-AU ;
    dct:hasPart C2024A00059:91 ;
    dct:isPartOf C2024A00059:79 ;
    dct:isReferencedBy C2024A00059: ;
    rdfs:comment "Subdivision CAppropriation - Abrievated Graph Key: S90"@en-AU ;
    skos:broader C2024A00059:91 ;
    skos:definition "Subdivision CAppropriation"@en-AU ;
    skos:narrower C2024A00059:79 ;
    skos:prefLabel "Subdivision S90"@en-AU ;
    dcat:accessURL <https://www.legislation.gov.au/C2024A00059/asmade/2024-07-09/text/original/epub/OEBPS/document_1/document_1.html#_Toc171508645> ;
    dcat:landingPage "https://www.legislation.gov.au/C2024A00059/asmade/2024-07-09/text/original/epub/OEBPS/document_1/document_1.html#_Toc171508645"^^xsd:anyURI ;
    dcat:theme legcons:Subdivision .

C2024A00059:93 a legcons:Division,
        owl:Class,
        dcat:Resource ;
    rdfs:label "Division - D93 Division 1 Simplified outline of this Part"@en-AU ;
    dct:hasPart C2024A00059:94 ;
    dct:isPartOf C2024A00059:92 ;
    dct:isReferencedBy C2024A00059: ;
    rdfs:comment "Division 1 Simplified outline of this Part - Abrievated Graph Key: D93"@en-AU ;
    skos:broader C2024A00059:94 ;
    skos:definition "Division 1 Simplified outline of this Part"@en-AU ;
    skos:narrower C2024A00059:92 ;
    skos:prefLabel "Division D93"@en-AU ;
    dcat:accessURL <https://www.legislation.gov.au/C2024A00059/asmade/2024-07-09/text/original/epub/OEBPS/document_1/document_1.html#_Toc171508648> ;
    dcat:landingPage "https://www.legislation.gov.au/C2024A00059/asmade/2024-07-09/text/original/epub/OEBPS/document_1/document_1.html#_Toc171508648"^^xsd:anyURI ;
    dcat:theme legcons:Division .

C2024A00059:100 a legcons:Division,
        owl:Class,
        dcat:Resource ;
    rdfs:label "Division - D100 Division 3 Information management"@en-AU ;
    dct:hasPart C2024A00059:101,
        C2024A00059:115 ;
    dct:isPartOf C2024A00059:92 ;
    dct:isReferencedBy C2024A00059: ;
    rdfs:comment "Division 3 Information management - Abrievated Graph Key: D100"@en-AU ;
    skos:broader C2024A00059:101,
        C2024A00059:115 ;
    skos:definition "Division 3 Information management"@en-AU ;
    skos:narrower C2024A00059:92 ;
    skos:prefLabel "Division D100"@en-AU ;
    dcat:accessURL <https://www.legislation.gov.au/C2024A00059/asmade/2024-07-09/text/original/epub/OEBPS/document_1/document_1.html#_Toc171508655> ;
    dcat:landingPage "https://www.legislation.gov.au/C2024A00059/asmade/2024-07-09/text/original/epub/OEBPS/document_1/document_1.html#_Toc171508655"^^xsd:anyURI ;
    dcat:theme legcons:Division .

C2024A00059:115 a legcons:Subdivision,
        owl:Class,
        dcat:Resource ;
    rdfs:label "Subdivision - S115 Subdivision BProtected information"@en-AU ;
    dct:hasPart C2024A00059:116,
        C2024A00059:117 ;
    dct:isPartOf C2024A00059:100 ;
    dct:isReferencedBy C2024A00059: ;
    rdfs:comment "Subdivision BProtected information - Abrievated Graph Key: S115"@en-AU ;
    skos:broader C2024A00059:116,
        C2024A00059:117 ;
    skos:definition "Subdivision BProtected information"@en-AU ;
    skos:narrower C2024A00059:100 ;
    skos:prefLabel "Subdivision S115"@en-AU ;
    dcat:accessURL <https://www.legislation.gov.au/C2024A00059/asmade/2024-07-09/text/original/epub/OEBPS/document_1/document_1.html#_Toc171508670> ;
    dcat:landingPage "https://www.legislation.gov.au/C2024A00059/asmade/2024-07-09/text/original/epub/OEBPS/document_1/document_1.html#_Toc171508670"^^xsd:anyURI ;
    dcat:theme legcons:Subdivision .

C2024A00059:121 a legcons:Division,
        owl:Class,
        dcat:Resource ;
    rdfs:label "Division - D121 Division 2 Reconsideration and review of decisions"@en-AU ;
    dct:hasPart C2024A00059:122,
        C2024A00059:123 ;
    dct:isPartOf C2024A00059:118 ;
    dct:isReferencedBy C2024A00059: ;
    rdfs:comment "Division 2 Reconsideration and review of decisions - Abrievated Graph Key: D121"@en-AU ;
    skos:broader C2024A00059:122,
        C2024A00059:123 ;
    skos:definition "Division 2 Reconsideration and review of decisions"@en-AU ;
    skos:narrower C2024A00059:118 ;
    skos:prefLabel "Division D121"@en-AU ;
    dcat:accessURL <https://www.legislation.gov.au/C2024A00059/asmade/2024-07-09/text/original/epub/OEBPS/document_1/document_1.html#_Toc171508676> ;
    dcat:landingPage "https://www.legislation.gov.au/C2024A00059/asmade/2024-07-09/text/original/epub/OEBPS/document_1/document_1.html#_Toc171508676"^^xsd:anyURI ;
    dcat:theme legcons:Division .

C2024A00059:124 a legcons:Division,
        owl:Class,
        dcat:Resource ;
    rdfs:label "Division - D124 Division 3 Recoverable payments"@en-AU ;
    dct:hasPart C2024A00059:125,
        C2024A00059:126 ;
    dct:isPartOf C2024A00059:118 ;
    dct:isReferencedBy C2024A00059: ;
    rdfs:comment "Division 3 Recoverable payments - Abrievated Graph Key: D124"@en-AU ;
    skos:broader C2024A00059:125,
        C2024A00059:126 ;
    skos:definition "Division 3 Recoverable payments"@en-AU ;
    skos:narrower C2024A00059:118 ;
    skos:prefLabel "Division D124"@en-AU ;
    dcat:accessURL <https://www.legislation.gov.au/C2024A00059/asmade/2024-07-09/text/original/epub/OEBPS/document_1/document_1.html#_Toc171508679> ;
    dcat:landingPage "https://www.legislation.gov.au/C2024A00059/asmade/2024-07-09/text/original/epub/OEBPS/document_1/document_1.html#_Toc171508679"^^xsd:anyURI ;
    dcat:theme legcons:Division .

C2024A00059:92 a legcons:Part,
        owl:Class,
        dcat:Resource ;
    rdfs:label "Part - P92 Part 5 Funding and information management for the National Residue Survey"@en-AU ;
    dct:hasPart C2024A00059:100,
        C2024A00059:93,
        C2024A00059:95 ;
    dct:isReferencedBy C2024A00059: ;
    rdfs:comment "Part 5 Funding and information management for the National Residue Survey - Abrievated Graph Key: P92"@en-AU ;
    skos:broader C2024A00059:100,
        C2024A00059:93,
        C2024A00059:95 ;
    skos:definition "Part 5 Funding and information management for the National Residue Survey"@en-AU ;
    skos:prefLabel "Part P92"@en-AU ;
    dcat:accessURL <https://www.legislation.gov.au/C2024A00059/asmade/2024-07-09/text/original/epub/OEBPS/document_1/document_1.html#_Toc171508647> ;
    dcat:landingPage "https://www.legislation.gov.au/C2024A00059/asmade/2024-07-09/text/original/epub/OEBPS/document_1/document_1.html#_Toc171508647"^^xsd:anyURI ;
    dcat:theme legcons:Part .

C2024A00059:118 a legcons:Part,
        owl:Class,
        dcat:Resource ;
    rdfs:label "Part - P118 Part 6 Other matters"@en-AU ;
    dct:hasPart C2024A00059:119,
        C2024A00059:121,
        C2024A00059:124,
        C2024A00059:127 ;
    dct:isReferencedBy C2024A00059: ;
    rdfs:comment "Part 6 Other matters - Abrievated Graph Key: P118"@en-AU ;
    skos:broader C2024A00059:119,
        C2024A00059:121,
        C2024A00059:124,
        C2024A00059:127 ;
    skos:definition "Part 6 Other matters"@en-AU ;
    skos:prefLabel "Part P118"@en-AU ;
    dcat:accessURL <https://www.legislation.gov.au/C2024A00059/asmade/2024-07-09/text/original/epub/OEBPS/document_1/document_1.html#_Toc171508673> ;
    dcat:landingPage "https://www.legislation.gov.au/C2024A00059/asmade/2024-07-09/text/original/epub/OEBPS/document_1/document_1.html#_Toc171508673"^^xsd:anyURI ;
    dcat:theme legcons:Part .

C2024A00059:127 a legcons:Division,
        owl:Class,
        dcat:Resource ;
    rdfs:label "Division - D127 Division 4 Administrative provisions"@en-AU ;
    dct:hasPart C2024A00059:128,
        C2024A00059:129,
        C2024A00059:130 ;
    dct:isPartOf C2024A00059:118 ;
    dct:isReferencedBy C2024A00059: ;
    rdfs:comment "Division 4 Administrative provisions - Abrievated Graph Key: D127"@en-AU ;
    skos:broader C2024A00059:128,
        C2024A00059:129,
        C2024A00059:130 ;
    skos:definition "Division 4 Administrative provisions"@en-AU ;
    skos:narrower C2024A00059:118 ;
    skos:prefLabel "Division D127"@en-AU ;
    dcat:accessURL <https://www.legislation.gov.au/C2024A00059/asmade/2024-07-09/text/original/epub/OEBPS/document_1/document_1.html#_Toc171508682> ;
    dcat:landingPage "https://www.legislation.gov.au/C2024A00059/asmade/2024-07-09/text/original/epub/OEBPS/document_1/document_1.html#_Toc171508682"^^xsd:anyURI ;
    dcat:theme legcons:Division .

C2024A00059:19 a legcons:Subdivision,
        owl:Class,
        dcat:Resource ;
    rdfs:label "Subdivision - S19 Subdivision ACommonwealth to make levy or charge payments"@en-AU ;
    dct:hasPart C2024A00059:20,
        C2024A00059:21,
        C2024A00059:22 ;
    dct:isPartOf C2024A00059:15 ;
    dct:isReferencedBy C2024A00059: ;
    rdfs:comment "Subdivision ACommonwealth to make levy or charge payments - Abrievated Graph Key: S19"@en-AU ;
    skos:broader C2024A00059:20,
        C2024A00059:21,
        C2024A00059:22 ;
    skos:definition "Subdivision ACommonwealth to make levy or charge payments"@en-AU ;
    skos:narrower C2024A00059:15 ;
    skos:prefLabel "Subdivision S19"@en-AU ;
    dcat:accessURL <https://www.legislation.gov.au/C2024A00059/asmade/2024-07-09/text/original/epub/OEBPS/document_1/document_1.html#_Toc171508574> ;
    dcat:landingPage "https://www.legislation.gov.au/C2024A00059/asmade/2024-07-09/text/original/epub/OEBPS/document_1/document_1.html#_Toc171508574"^^xsd:anyURI ;
    dcat:theme legcons:Subdivision .

C2024A00059:63 a legcons:Division,
        owl:Class,
        dcat:Resource ;
    rdfs:label "Division - D63 Division 2 Funding for Animal Health Australia"@en-AU ;
    dct:hasPart C2024A00059:64,
        C2024A00059:69,
        C2024A00059:74 ;
    dct:isPartOf C2024A00059:60 ;
    dct:isReferencedBy C2024A00059: ;
    rdfs:comment "Division 2 Funding for Animal Health Australia - Abrievated Graph Key: D63"@en-AU ;
    skos:broader C2024A00059:64,
        C2024A00059:69,
        C2024A00059:74 ;
    skos:definition "Division 2 Funding for Animal Health Australia"@en-AU ;
    skos:narrower C2024A00059:60 ;
    skos:prefLabel "Division D63"@en-AU ;
    dcat:accessURL <https://www.legislation.gov.au/C2024A00059/asmade/2024-07-09/text/original/epub/OEBPS/document_1/document_1.html#_Toc171508618> ;
    dcat:landingPage "https://www.legislation.gov.au/C2024A00059/asmade/2024-07-09/text/original/epub/OEBPS/document_1/document_1.html#_Toc171508618"^^xsd:anyURI ;
    dcat:theme legcons:Division .

C2024A00059:79 a legcons:Division,
        owl:Class,
        dcat:Resource ;
    rdfs:label "Division - D79 Division 2 Funding for Plant Health Australia"@en-AU ;
    dct:hasPart C2024A00059:80,
        C2024A00059:85,
        C2024A00059:90 ;
    dct:isPartOf C2024A00059:76 ;
    dct:isReferencedBy C2024A00059: ;
    rdfs:comment "Division 2 Funding for Plant Health Australia - Abrievated Graph Key: D79"@en-AU ;
    skos:broader C2024A00059:80,
        C2024A00059:85,
        C2024A00059:90 ;
    skos:definition "Division 2 Funding for Plant Health Australia"@en-AU ;
    skos:narrower C2024A00059:76 ;
    skos:prefLabel "Division D79"@en-AU ;
    dcat:accessURL <https://www.legislation.gov.au/C2024A00059/asmade/2024-07-09/text/original/epub/OEBPS/document_1/document_1.html#_Toc171508634> ;
    dcat:landingPage "https://www.legislation.gov.au/C2024A00059/asmade/2024-07-09/text/original/epub/OEBPS/document_1/document_1.html#_Toc171508634"^^xsd:anyURI ;
    dcat:theme legcons:Division .

C2024A00059:64 a legcons:Subdivision,
        owl:Class,
        dcat:Resource ;
    rdfs:label "Subdivision - S64 Subdivision APayments relating to biosecurity activity"@en-AU ;
    dct:hasPart C2024A00059:65,
        C2024A00059:66,
        C2024A00059:67,
        C2024A00059:68 ;
    dct:isPartOf C2024A00059:63 ;
    dct:isReferencedBy C2024A00059: ;
    rdfs:comment "Subdivision APayments relating to biosecurity activity - Abrievated Graph Key: S64"@en-AU ;
    skos:broader C2024A00059:65,
        C2024A00059:66,
        C2024A00059:67,
        C2024A00059:68 ;
    skos:definition "Subdivision APayments relating to biosecurity activity"@en-AU ;
    skos:narrower C2024A00059:63 ;
    skos:prefLabel "Subdivision S64"@en-AU ;
    dcat:accessURL <https://www.legislation.gov.au/C2024A00059/asmade/2024-07-09/text/original/epub/OEBPS/document_1/document_1.html#_Toc171508619> ;
    dcat:landingPage "https://www.legislation.gov.au/C2024A00059/asmade/2024-07-09/text/original/epub/OEBPS/document_1/document_1.html#_Toc171508619"^^xsd:anyURI ;
    dcat:theme legcons:Subdivision .

C2024A00059:69 a legcons:Subdivision,
        owl:Class,
        dcat:Resource ;
    rdfs:label "Subdivision - S69 Subdivision BPayments relating to biosecurity response"@en-AU ;
    dct:hasPart C2024A00059:70,
        C2024A00059:71,
        C2024A00059:72,
        C2024A00059:73 ;
    dct:isPartOf C2024A00059:63 ;
    dct:isReferencedBy C2024A00059: ;
    rdfs:comment "Subdivision BPayments relating to biosecurity response - Abrievated Graph Key: S69"@en-AU ;
    skos:broader C2024A00059:70,
        C2024A00059:71,
        C2024A00059:72,
        C2024A00059:73 ;
    skos:definition "Subdivision BPayments relating to biosecurity response"@en-AU ;
    skos:narrower C2024A00059:63 ;
    skos:prefLabel "Subdivision S69"@en-AU ;
    dcat:accessURL <https://www.legislation.gov.au/C2024A00059/asmade/2024-07-09/text/original/epub/OEBPS/document_1/document_1.html#_Toc171508624> ;
    dcat:landingPage "https://www.legislation.gov.au/C2024A00059/asmade/2024-07-09/text/original/epub/OEBPS/document_1/document_1.html#_Toc171508624"^^xsd:anyURI ;
    dcat:theme legcons:Subdivision .

C2024A00059:80 a legcons:Subdivision,
        owl:Class,
        dcat:Resource ;
    rdfs:label "Subdivision - S80 Subdivision APayments relating to biosecurity activity"@en-AU ;
    dct:hasPart C2024A00059:81,
        C2024A00059:82,
        C2024A00059:83,
        C2024A00059:84 ;
    dct:isPartOf C2024A00059:79 ;
    dct:isReferencedBy C2024A00059: ;
    rdfs:comment "Subdivision APayments relating to biosecurity activity - Abrievated Graph Key: S80"@en-AU ;
    skos:broader C2024A00059:81,
        C2024A00059:82,
        C2024A00059:83,
        C2024A00059:84 ;
    skos:definition "Subdivision APayments relating to biosecurity activity"@en-AU ;
    skos:narrower C2024A00059:79 ;
    skos:prefLabel "Subdivision S80"@en-AU ;
    dcat:accessURL <https://www.legislation.gov.au/C2024A00059/asmade/2024-07-09/text/original/epub/OEBPS/document_1/document_1.html#_Toc171508635> ;
    dcat:landingPage "https://www.legislation.gov.au/C2024A00059/asmade/2024-07-09/text/original/epub/OEBPS/document_1/document_1.html#_Toc171508635"^^xsd:anyURI ;
    dcat:theme legcons:Subdivision .

C2024A00059:85 a legcons:Subdivision,
        owl:Class,
        dcat:Resource ;
    rdfs:label "Subdivision - S85 Subdivision BPayments relating to biosecurity response"@en-AU ;
    dct:hasPart C2024A00059:86,
        C2024A00059:87,
        C2024A00059:88,
        C2024A00059:89 ;
    dct:isPartOf C2024A00059:79 ;
    dct:isReferencedBy C2024A00059: ;
    rdfs:comment "Subdivision BPayments relating to biosecurity response - Abrievated Graph Key: S85"@en-AU ;
    skos:broader C2024A00059:86,
        C2024A00059:87,
        C2024A00059:88,
        C2024A00059:89 ;
    skos:definition "Subdivision BPayments relating to biosecurity response"@en-AU ;
    skos:narrower C2024A00059:79 ;
    skos:prefLabel "Subdivision S85"@en-AU ;
    dcat:accessURL <https://www.legislation.gov.au/C2024A00059/asmade/2024-07-09/text/original/epub/OEBPS/document_1/document_1.html#_Toc171508640> ;
    dcat:landingPage "https://www.legislation.gov.au/C2024A00059/asmade/2024-07-09/text/original/epub/OEBPS/document_1/document_1.html#_Toc171508640"^^xsd:anyURI ;
    dcat:theme legcons:Subdivision .

C2024A00059:95 a legcons:Division,
        owl:Class,
        dcat:Resource ;
    rdfs:label "Division - D95 Division 2 Funding for National Residue Survey"@en-AU ;
    dct:hasPart C2024A00059:96,
        C2024A00059:97,
        C2024A00059:98,
        C2024A00059:99 ;
    dct:isPartOf C2024A00059:92 ;
    dct:isReferencedBy C2024A00059: ;
    rdfs:comment "Division 2 Funding for National Residue Survey - Abrievated Graph Key: D95"@en-AU ;
    skos:broader C2024A00059:96,
        C2024A00059:97,
        C2024A00059:98,
        C2024A00059:99 ;
    skos:definition "Division 2 Funding for National Residue Survey"@en-AU ;
    skos:narrower C2024A00059:92 ;
    skos:prefLabel "Division D95"@en-AU ;
    dcat:accessURL <https://www.legislation.gov.au/C2024A00059/asmade/2024-07-09/text/original/epub/OEBPS/document_1/document_1.html#_Toc171508650> ;
    dcat:landingPage "https://www.legislation.gov.au/C2024A00059/asmade/2024-07-09/text/original/epub/OEBPS/document_1/document_1.html#_Toc171508650"^^xsd:anyURI ;
    dcat:theme legcons:Division .

C2024A00059:1 a legcons:Part,
        owl:Class,
        dcat:Resource ;
    rdfs:label "Part - P1 Part 1 Preliminary"@en-AU ;
    dct:hasPart C2024A00059:10,
        C2024A00059:11,
        C2024A00059:12,
        C2024A00059:13,
        C2024A00059:14,
        C2024A00059:2,
        C2024A00059:3,
        C2024A00059:4,
        C2024A00059:5,
        C2024A00059:6,
        C2024A00059:7,
        C2024A00059:8,
        C2024A00059:9 ;
    dct:isReferencedBy C2024A00059: ;
    rdfs:comment "Part 1 Preliminary - Abrievated Graph Key: P1"@en-AU ;
    skos:broader C2024A00059:10,
        C2024A00059:11,
        C2024A00059:12,
        C2024A00059:13,
        C2024A00059:14,
        C2024A00059:2,
        C2024A00059:3,
        C2024A00059:4,
        C2024A00059:5,
        C2024A00059:6,
        C2024A00059:7,
        C2024A00059:8,
        C2024A00059:9 ;
    skos:definition "Part 1 Preliminary"@en-AU ;
    skos:prefLabel "Part P1"@en-AU ;
    dcat:accessURL <https://www.legislation.gov.au/C2024A00059/asmade/2024-07-09/text/original/epub/OEBPS/document_1/document_1.html#_Toc171508556> ;
    dcat:landingPage "https://www.legislation.gov.au/C2024A00059/asmade/2024-07-09/text/original/epub/OEBPS/document_1/document_1.html#_Toc171508556"^^xsd:anyURI ;
    dcat:theme legcons:Part .

C2024A00059:101 a legcons:Subdivision,
        owl:Class,
        dcat:Resource ;
    rdfs:label "Subdivision - S101 Subdivision AAuthorised uses and disclosures of relevant NRS information"@en-AU ;
    dct:hasPart C2024A00059:102,
        C2024A00059:103,
        C2024A00059:104,
        C2024A00059:105,
        C2024A00059:106,
        C2024A00059:107,
        C2024A00059:108,
        C2024A00059:109,
        C2024A00059:110,
        C2024A00059:111,
        C2024A00059:112,
        C2024A00059:113,
        C2024A00059:114 ;
    dct:isPartOf C2024A00059:100 ;
    dct:isReferencedBy C2024A00059: ;
    rdfs:comment "Subdivision AAuthorised uses and disclosures of relevant NRS information - Abrievated Graph Key: S101"@en-AU ;
    skos:broader C2024A00059:102,
        C2024A00059:103,
        C2024A00059:104,
        C2024A00059:105,
        C2024A00059:106,
        C2024A00059:107,
        C2024A00059:108,
        C2024A00059:109,
        C2024A00059:110,
        C2024A00059:111,
        C2024A00059:112,
        C2024A00059:113,
        C2024A00059:114 ;
    skos:definition "Subdivision AAuthorised uses and disclosures of relevant NRS information"@en-AU ;
    skos:narrower C2024A00059:100 ;
    skos:prefLabel "Subdivision S101"@en-AU ;
    dcat:accessURL <https://www.legislation.gov.au/C2024A00059/asmade/2024-07-09/text/original/epub/OEBPS/document_1/document_1.html#_Toc171508656> ;
    dcat:landingPage "https://www.legislation.gov.au/C2024A00059/asmade/2024-07-09/text/original/epub/OEBPS/document_1/document_1.html#_Toc171508656"^^xsd:anyURI ;
    dcat:theme legcons:Subdivision .

C2024A00059:15 a legcons:Part,
        owl:Class,
        dcat:Resource ;
    rdfs:label "Part - P15 Part 2 Funding for recipient bodies"@en-AU ;
    dct:hasPart C2024A00059:16,
        C2024A00059:18,
        C2024A00059:19,
        C2024A00059:23,
        C2024A00059:24,
        C2024A00059:25,
        C2024A00059:26,
        C2024A00059:27,
        C2024A00059:28,
        C2024A00059:29,
        C2024A00059:30,
        C2024A00059:31,
        C2024A00059:32,
        C2024A00059:33,
        C2024A00059:34,
        C2024A00059:35,
        C2024A00059:36,
        C2024A00059:37,
        C2024A00059:38,
        C2024A00059:39,
        C2024A00059:40,
        C2024A00059:41,
        C2024A00059:42,
        C2024A00059:43,
        C2024A00059:44,
        C2024A00059:45,
        C2024A00059:46,
        C2024A00059:47,
        C2024A00059:48,
        C2024A00059:49,
        C2024A00059:50,
        C2024A00059:51,
        C2024A00059:52,
        C2024A00059:53,
        C2024A00059:54,
        C2024A00059:55,
        C2024A00059:56,
        C2024A00059:57,
        C2024A00059:58,
        C2024A00059:59 ;
    dct:isReferencedBy C2024A00059: ;
    rdfs:comment "Part 2 Funding for recipient bodies - Abrievated Graph Key: P15"@en-AU ;
    skos:broader C2024A00059:16,
        C2024A00059:18,
        C2024A00059:19,
        C2024A00059:23,
        C2024A00059:24,
        C2024A00059:25,
        C2024A00059:26,
        C2024A00059:27,
        C2024A00059:28,
        C2024A00059:29,
        C2024A00059:30,
        C2024A00059:31,
        C2024A00059:32,
        C2024A00059:33,
        C2024A00059:34,
        C2024A00059:35,
        C2024A00059:36,
        C2024A00059:37,
        C2024A00059:38,
        C2024A00059:39,
        C2024A00059:40,
        C2024A00059:41,
        C2024A00059:42,
        C2024A00059:43,
        C2024A00059:44,
        C2024A00059:45,
        C2024A00059:46,
        C2024A00059:47,
        C2024A00059:48,
        C2024A00059:49,
        C2024A00059:50,
        C2024A00059:51,
        C2024A00059:52,
        C2024A00059:53,
        C2024A00059:54,
        C2024A00059:55,
        C2024A00059:56,
        C2024A00059:57,
        C2024A00059:58,
        C2024A00059:59 ;
    skos:definition "Part 2 Funding for recipient bodies"@en-AU ;
    skos:prefLabel "Part P15"@en-AU ;
    dcat:accessURL <https://www.legislation.gov.au/C2024A00059/asmade/2024-07-09/text/original/epub/OEBPS/document_1/document_1.html#_Toc171508570> ;
    dcat:landingPage "https://www.legislation.gov.au/C2024A00059/asmade/2024-07-09/text/original/epub/OEBPS/document_1/document_1.html#_Toc171508570"^^xsd:anyURI ;
    dcat:theme legcons:Part .

C2024A00059: a owl:Class,
        dcat:Dataset,
        dcat:Resource ;
    rdfs:label "Primary Industries Levies and Charges Disbursement Act 2024" ;
    dct:Jurisdiction " Department of Agriculture, Fisheries and Forestry "@en-AU ;
    dct:created "2024-08-30T15:23:08.648963"^^xsd:dateTime ;
    dct:creator "https://orcid.org/0009-0007-8434-7325"^^xsd:anyURI ;
    dct:date "2024-07-09T00:00:00+10:00"^^xsd:dateTime ;
    dct:description "Primary Industries Levies and Charges Disbursement Act 2024"@en-AU ;
    dct:identifier "https://www.legislation.gov.au/C2024A00059/asmade"^^xsd:anyURI ;
    dct:license <https://creativecommons.org/licenses/by-sa/4.0/> ;
    dct:source "scheme=AGLSTERMS.AglsAgent; corporateName=Office Parliamentary Counsel; address=Locked Bag 30 Kingston ACT 2604; contact=+61 2 6120 1400"@en-AU ;
    dct:subject "Primary Industries Levies and Charges Disbursement Act 2024"@en-AU ;
    dct:title "Primary Industries Levies and Charges Disbursement Act 2024"@en-AU ;
    owl:imports legcons: ;
    dcat:theme legcons:Division,
        legcons:Item,
        legcons:Part,
        legcons:Subdivision ;
    schema:identifier "C2024A00059" ;
    schema:status "In force" ;
    schema:version "C2024A00059" .

