@prefix C2020A00012: <http://example.org/au/leg/dataset/C2020A00012/> .
@prefix dcat: <http://www.w3.org/ns/dcat#> .
@prefix dct: <http://purl.org/dc/terms/> .
@prefix legcons: <http://example.org/au/leg/concepts/> .
@prefix owl: <http://www.w3.org/2002/07/owl#> .
@prefix rdfs: <http://www.w3.org/2000/01/rdf-schema#> .
@prefix schema: <https://schema.org/> .
@prefix skos: <http://www.w3.org/2004/02/skos/core#> .
@prefix xsd: <http://www.w3.org/2001/XMLSchema#> .

C2020A00012:10 a legcons:Item,
        owl:Class,
        dcat:Resource ;
    rdfs:label "Item - I10 8  Extension of this Act to external Territories and other areas"@en-AU ;
    dct:isPartOf C2020A00012:1 ;
    dct:isReferencedBy C2020A00012: ;
    rdfs:comment "8  Extension of this Act to external Territories and other areas - Abrievated Graph Key: I10"@en-AU ;
    skos:definition "8  Extension of this Act to external Territories and other areas"@en-AU ;
    skos:narrower C2020A00012:1 ;
    skos:prefLabel "Item I10"@en-AU ;
    dcat:accessURL <https://www.legislation.gov.au/C2020A00012/2024-07-10/2024-07-10/text/original/epub/OEBPS/document_1/document_1.html#_Toc172118702> ;
    dcat:landingPage "https://www.legislation.gov.au/C2020A00012/2024-07-10/2024-07-10/text/original/epub/OEBPS/document_1/document_1.html#_Toc172118702"^^xsd:anyURI ;
    dcat:theme legcons:Item .

C2020A00012:102 a legcons:Item,
        owl:Class,
        dcat:Resource ;
    rdfs:label "Item - I102 77  Simplified outline of this Chapter"@en-AU ;
    dct:isPartOf C2020A00012:101 ;
    dct:isReferencedBy C2020A00012: ;
    rdfs:comment "77  Simplified outline of this Chapter - Abrievated Graph Key: I102"@en-AU ;
    skos:definition "77  Simplified outline of this Chapter"@en-AU ;
    skos:narrower C2020A00012:101 ;
    skos:prefLabel "Item I102"@en-AU ;
    dcat:accessURL <https://www.legislation.gov.au/C2020A00012/2024-07-10/2024-07-10/text/original/epub/OEBPS/document_1/document_1.html#_Toc172118794> ;
    dcat:landingPage "https://www.legislation.gov.au/C2020A00012/2024-07-10/2024-07-10/text/original/epub/OEBPS/document_1/document_1.html#_Toc172118794"^^xsd:anyURI ;
    dcat:theme legcons:Item .

C2020A00012:104 a legcons:Item,
        owl:Class,
        dcat:Resource ;
    rdfs:label "Item - I104 78  Application for accreditation of property"@en-AU ;
    dct:isPartOf C2020A00012:103 ;
    dct:isReferencedBy C2020A00012: ;
    rdfs:comment "78  Application for accreditation of property - Abrievated Graph Key: I104"@en-AU ;
    skos:definition "78  Application for accreditation of property"@en-AU ;
    skos:narrower C2020A00012:103 ;
    skos:prefLabel "Item I104"@en-AU ;
    dcat:accessURL <https://www.legislation.gov.au/C2020A00012/2024-07-10/2024-07-10/text/original/epub/OEBPS/document_1/document_1.html#_Toc172118796> ;
    dcat:landingPage "https://www.legislation.gov.au/C2020A00012/2024-07-10/2024-07-10/text/original/epub/OEBPS/document_1/document_1.html#_Toc172118796"^^xsd:anyURI ;
    dcat:theme legcons:Item .

C2020A00012:105 a legcons:Item,
        owl:Class,
        dcat:Resource ;
    rdfs:label "Item - I105 79  Secretary must decide whether to accredit property"@en-AU ;
    dct:isPartOf C2020A00012:103 ;
    dct:isReferencedBy C2020A00012: ;
    rdfs:comment "79  Secretary must decide whether to accredit property - Abrievated Graph Key: I105"@en-AU ;
    skos:definition "79  Secretary must decide whether to accredit property"@en-AU ;
    skos:narrower C2020A00012:103 ;
    skos:prefLabel "Item I105"@en-AU ;
    dcat:accessURL <https://www.legislation.gov.au/C2020A00012/2024-07-10/2024-07-10/text/original/epub/OEBPS/document_1/document_1.html#_Toc172118797> ;
    dcat:landingPage "https://www.legislation.gov.au/C2020A00012/2024-07-10/2024-07-10/text/original/epub/OEBPS/document_1/document_1.html#_Toc172118797"^^xsd:anyURI ;
    dcat:theme legcons:Item .

C2020A00012:106 a legcons:Item,
        owl:Class,
        dcat:Resource ;
    rdfs:label "Item - I106 80  Conditions of accreditation"@en-AU ;
    dct:isPartOf C2020A00012:103 ;
    dct:isReferencedBy C2020A00012: ;
    rdfs:comment "80  Conditions of accreditation - Abrievated Graph Key: I106"@en-AU ;
    skos:definition "80  Conditions of accreditation"@en-AU ;
    skos:narrower C2020A00012:103 ;
    skos:prefLabel "Item I106"@en-AU ;
    dcat:accessURL <https://www.legislation.gov.au/C2020A00012/2024-07-10/2024-07-10/text/original/epub/OEBPS/document_1/document_1.html#_Toc172118798> ;
    dcat:landingPage "https://www.legislation.gov.au/C2020A00012/2024-07-10/2024-07-10/text/original/epub/OEBPS/document_1/document_1.html#_Toc172118798"^^xsd:anyURI ;
    dcat:theme legcons:Item .

C2020A00012:107 a legcons:Item,
        owl:Class,
        dcat:Resource ;
    rdfs:label "Item - I107 81  Notice of decision"@en-AU ;
    dct:isPartOf C2020A00012:103 ;
    dct:isReferencedBy C2020A00012: ;
    rdfs:comment "81  Notice of decision - Abrievated Graph Key: I107"@en-AU ;
    skos:definition "81  Notice of decision"@en-AU ;
    skos:narrower C2020A00012:103 ;
    skos:prefLabel "Item I107"@en-AU ;
    dcat:accessURL <https://www.legislation.gov.au/C2020A00012/2024-07-10/2024-07-10/text/original/epub/OEBPS/document_1/document_1.html#_Toc172118799> ;
    dcat:landingPage "https://www.legislation.gov.au/C2020A00012/2024-07-10/2024-07-10/text/original/epub/OEBPS/document_1/document_1.html#_Toc172118799"^^xsd:anyURI ;
    dcat:theme legcons:Item .

C2020A00012:108 a legcons:Item,
        owl:Class,
        dcat:Resource ;
    rdfs:label "Item - I108 82  Period of effect of accreditation"@en-AU ;
    dct:isPartOf C2020A00012:103 ;
    dct:isReferencedBy C2020A00012: ;
    rdfs:comment "82  Period of effect of accreditation - Abrievated Graph Key: I108"@en-AU ;
    skos:definition "82  Period of effect of accreditation"@en-AU ;
    skos:narrower C2020A00012:103 ;
    skos:prefLabel "Item I108"@en-AU ;
    dcat:accessURL <https://www.legislation.gov.au/C2020A00012/2024-07-10/2024-07-10/text/original/epub/OEBPS/document_1/document_1.html#_Toc172118800> ;
    dcat:landingPage "https://www.legislation.gov.au/C2020A00012/2024-07-10/2024-07-10/text/original/epub/OEBPS/document_1/document_1.html#_Toc172118800"^^xsd:anyURI ;
    dcat:theme legcons:Item .

C2020A00012:11 a legcons:Item,
        owl:Class,
        dcat:Resource ;
    rdfs:label "Item - I11 9  Application of this Act in external Territories and other areas"@en-AU ;
    dct:isPartOf C2020A00012:1 ;
    dct:isReferencedBy C2020A00012: ;
    rdfs:comment "9  Application of this Act in external Territories and other areas - Abrievated Graph Key: I11"@en-AU ;
    skos:definition "9  Application of this Act in external Territories and other areas"@en-AU ;
    skos:narrower C2020A00012:1 ;
    skos:prefLabel "Item I11"@en-AU ;
    dcat:accessURL <https://www.legislation.gov.au/C2020A00012/2024-07-10/2024-07-10/text/original/epub/OEBPS/document_1/document_1.html#_Toc172118703> ;
    dcat:landingPage "https://www.legislation.gov.au/C2020A00012/2024-07-10/2024-07-10/text/original/epub/OEBPS/document_1/document_1.html#_Toc172118703"^^xsd:anyURI ;
    dcat:theme legcons:Item .

C2020A00012:110 a legcons:Item,
        owl:Class,
        dcat:Resource ;
    rdfs:label "Item - I110 83  Application to renew accreditation of property"@en-AU ;
    dct:isPartOf C2020A00012:109 ;
    dct:isReferencedBy C2020A00012: ;
    rdfs:comment "83  Application to renew accreditation of property - Abrievated Graph Key: I110"@en-AU ;
    skos:definition "83  Application to renew accreditation of property"@en-AU ;
    skos:narrower C2020A00012:109 ;
    skos:prefLabel "Item I110"@en-AU ;
    dcat:accessURL <https://www.legislation.gov.au/C2020A00012/2024-07-10/2024-07-10/text/original/epub/OEBPS/document_1/document_1.html#_Toc172118802> ;
    dcat:landingPage "https://www.legislation.gov.au/C2020A00012/2024-07-10/2024-07-10/text/original/epub/OEBPS/document_1/document_1.html#_Toc172118802"^^xsd:anyURI ;
    dcat:theme legcons:Item .

C2020A00012:111 a legcons:Item,
        owl:Class,
        dcat:Resource ;
    rdfs:label "Item - I111 84  Secretary must decide whether to renew accreditation"@en-AU ;
    dct:isPartOf C2020A00012:109 ;
    dct:isReferencedBy C2020A00012: ;
    rdfs:comment "84  Secretary must decide whether to renew accreditation - Abrievated Graph Key: I111"@en-AU ;
    skos:definition "84  Secretary must decide whether to renew accreditation"@en-AU ;
    skos:narrower C2020A00012:109 ;
    skos:prefLabel "Item I111"@en-AU ;
    dcat:accessURL <https://www.legislation.gov.au/C2020A00012/2024-07-10/2024-07-10/text/original/epub/OEBPS/document_1/document_1.html#_Toc172118803> ;
    dcat:landingPage "https://www.legislation.gov.au/C2020A00012/2024-07-10/2024-07-10/text/original/epub/OEBPS/document_1/document_1.html#_Toc172118803"^^xsd:anyURI ;
    dcat:theme legcons:Item .

C2020A00012:112 a legcons:Item,
        owl:Class,
        dcat:Resource ;
    rdfs:label "Item - I112 85  Conditions of renewed accreditation"@en-AU ;
    dct:isPartOf C2020A00012:109 ;
    dct:isReferencedBy C2020A00012: ;
    rdfs:comment "85  Conditions of renewed accreditation - Abrievated Graph Key: I112"@en-AU ;
    skos:definition "85  Conditions of renewed accreditation"@en-AU ;
    skos:narrower C2020A00012:109 ;
    skos:prefLabel "Item I112"@en-AU ;
    dcat:accessURL <https://www.legislation.gov.au/C2020A00012/2024-07-10/2024-07-10/text/original/epub/OEBPS/document_1/document_1.html#_Toc172118804> ;
    dcat:landingPage "https://www.legislation.gov.au/C2020A00012/2024-07-10/2024-07-10/text/original/epub/OEBPS/document_1/document_1.html#_Toc172118804"^^xsd:anyURI ;
    dcat:theme legcons:Item .

C2020A00012:113 a legcons:Item,
        owl:Class,
        dcat:Resource ;
    rdfs:label "Item - I113 86  Notice of decision"@en-AU ;
    dct:isPartOf C2020A00012:109 ;
    dct:isReferencedBy C2020A00012: ;
    rdfs:comment "86  Notice of decision - Abrievated Graph Key: I113"@en-AU ;
    skos:definition "86  Notice of decision"@en-AU ;
    skos:narrower C2020A00012:109 ;
    skos:prefLabel "Item I113"@en-AU ;
    dcat:accessURL <https://www.legislation.gov.au/C2020A00012/2024-07-10/2024-07-10/text/original/epub/OEBPS/document_1/document_1.html#_Toc172118805> ;
    dcat:landingPage "https://www.legislation.gov.au/C2020A00012/2024-07-10/2024-07-10/text/original/epub/OEBPS/document_1/document_1.html#_Toc172118805"^^xsd:anyURI ;
    dcat:theme legcons:Item .

C2020A00012:116 a legcons:Item,
        owl:Class,
        dcat:Resource ;
    rdfs:label "Item - I116 87  Application by manager for variation of accreditation or approval of alteration of property"@en-AU ;
    dct:isPartOf C2020A00012:115 ;
    dct:isReferencedBy C2020A00012: ;
    rdfs:comment "87  Application by manager for variation of accreditation or approval of alteration of property - Abrievated Graph Key: I116"@en-AU ;
    skos:definition "87  Application by manager for variation of accreditation or approval of alteration of property"@en-AU ;
    skos:narrower C2020A00012:115 ;
    skos:prefLabel "Item I116"@en-AU ;
    dcat:accessURL <https://www.legislation.gov.au/C2020A00012/2024-07-10/2024-07-10/text/original/epub/OEBPS/document_1/document_1.html#_Toc172118808> ;
    dcat:landingPage "https://www.legislation.gov.au/C2020A00012/2024-07-10/2024-07-10/text/original/epub/OEBPS/document_1/document_1.html#_Toc172118808"^^xsd:anyURI ;
    dcat:theme legcons:Item .

C2020A00012:117 a legcons:Item,
        owl:Class,
        dcat:Resource ;
    rdfs:label "Item - I117 88  Notice of variation or approval of alteration"@en-AU ;
    dct:isPartOf C2020A00012:115 ;
    dct:isReferencedBy C2020A00012: ;
    rdfs:comment "88  Notice of variation or approval of alteration - Abrievated Graph Key: I117"@en-AU ;
    skos:definition "88  Notice of variation or approval of alteration"@en-AU ;
    skos:narrower C2020A00012:115 ;
    skos:prefLabel "Item I117"@en-AU ;
    dcat:accessURL <https://www.legislation.gov.au/C2020A00012/2024-07-10/2024-07-10/text/original/epub/OEBPS/document_1/document_1.html#_Toc172118809> ;
    dcat:landingPage "https://www.legislation.gov.au/C2020A00012/2024-07-10/2024-07-10/text/original/epub/OEBPS/document_1/document_1.html#_Toc172118809"^^xsd:anyURI ;
    dcat:theme legcons:Item .

C2020A00012:118 a legcons:Item,
        owl:Class,
        dcat:Resource ;
    rdfs:label "Item - I118 89  Certain variations must not be made unless approved"@en-AU ;
    dct:isPartOf C2020A00012:115 ;
    dct:isReferencedBy C2020A00012: ;
    rdfs:comment "89  Certain variations must not be made unless approved - Abrievated Graph Key: I118"@en-AU ;
    skos:definition "89  Certain variations must not be made unless approved"@en-AU ;
    skos:narrower C2020A00012:115 ;
    skos:prefLabel "Item I118"@en-AU ;
    dcat:accessURL <https://www.legislation.gov.au/C2020A00012/2024-07-10/2024-07-10/text/original/epub/OEBPS/document_1/document_1.html#_Toc172118810> ;
    dcat:landingPage "https://www.legislation.gov.au/C2020A00012/2024-07-10/2024-07-10/text/original/epub/OEBPS/document_1/document_1.html#_Toc172118810"^^xsd:anyURI ;
    dcat:theme legcons:Item .

C2020A00012:12 a legcons:Item,
        owl:Class,
        dcat:Resource ;
    rdfs:label "Item - I12 10  Rights of foreign aircraft and vessels under Convention on the Law of the Sea not affected"@en-AU ;
    dct:isPartOf C2020A00012:1 ;
    dct:isReferencedBy C2020A00012: ;
    rdfs:comment "10  Rights of foreign aircraft and vessels under Convention on the Law of the Sea not affected - Abrievated Graph Key: I12"@en-AU ;
    skos:definition "10  Rights of foreign aircraft and vessels under Convention on the Law of the Sea not affected"@en-AU ;
    skos:narrower C2020A00012:1 ;
    skos:prefLabel "Item I12"@en-AU ;
    dcat:accessURL <https://www.legislation.gov.au/C2020A00012/2024-07-10/2024-07-10/text/original/epub/OEBPS/document_1/document_1.html#_Toc172118704> ;
    dcat:landingPage "https://www.legislation.gov.au/C2020A00012/2024-07-10/2024-07-10/text/original/epub/OEBPS/document_1/document_1.html#_Toc172118704"^^xsd:anyURI ;
    dcat:theme legcons:Item .

C2020A00012:120 a legcons:Item,
        owl:Class,
        dcat:Resource ;
    rdfs:label "Item - I120 90  Secretary may make variations in relation to accreditation"@en-AU ;
    dct:isPartOf C2020A00012:119 ;
    dct:isReferencedBy C2020A00012: ;
    rdfs:comment "90  Secretary may make variations in relation to accreditation - Abrievated Graph Key: I120"@en-AU ;
    skos:definition "90  Secretary may make variations in relation to accreditation"@en-AU ;
    skos:narrower C2020A00012:119 ;
    skos:prefLabel "Item I120"@en-AU ;
    dcat:accessURL <https://www.legislation.gov.au/C2020A00012/2024-07-10/2024-07-10/text/original/epub/OEBPS/document_1/document_1.html#_Toc172118812> ;
    dcat:landingPage "https://www.legislation.gov.au/C2020A00012/2024-07-10/2024-07-10/text/original/epub/OEBPS/document_1/document_1.html#_Toc172118812"^^xsd:anyURI ;
    dcat:theme legcons:Item .

C2020A00012:121 a legcons:Item,
        owl:Class,
        dcat:Resource ;
    rdfs:label "Item - I121 91  Notice of variation"@en-AU ;
    dct:isPartOf C2020A00012:119 ;
    dct:isReferencedBy C2020A00012: ;
    rdfs:comment "91  Notice of variation - Abrievated Graph Key: I121"@en-AU ;
    skos:definition "91  Notice of variation"@en-AU ;
    skos:narrower C2020A00012:119 ;
    skos:prefLabel "Item I121"@en-AU ;
    dcat:accessURL <https://www.legislation.gov.au/C2020A00012/2024-07-10/2024-07-10/text/original/epub/OEBPS/document_1/document_1.html#_Toc172118813> ;
    dcat:landingPage "https://www.legislation.gov.au/C2020A00012/2024-07-10/2024-07-10/text/original/epub/OEBPS/document_1/document_1.html#_Toc172118813"^^xsd:anyURI ;
    dcat:theme legcons:Item .

C2020A00012:124 a legcons:Item,
        owl:Class,
        dcat:Resource ;
    rdfs:label "Item - I124 92  Manager may request suspension"@en-AU ;
    dct:isPartOf C2020A00012:123 ;
    dct:isReferencedBy C2020A00012: ;
    rdfs:comment "92  Manager may request suspension - Abrievated Graph Key: I124"@en-AU ;
    skos:definition "92  Manager may request suspension"@en-AU ;
    skos:narrower C2020A00012:123 ;
    skos:prefLabel "Item I124"@en-AU ;
    dcat:accessURL <https://www.legislation.gov.au/C2020A00012/2024-07-10/2024-07-10/text/original/epub/OEBPS/document_1/document_1.html#_Toc172118816> ;
    dcat:landingPage "https://www.legislation.gov.au/C2020A00012/2024-07-10/2024-07-10/text/original/epub/OEBPS/document_1/document_1.html#_Toc172118816"^^xsd:anyURI ;
    dcat:theme legcons:Item .

C2020A00012:125 a legcons:Item,
        owl:Class,
        dcat:Resource ;
    rdfs:label "Item - I125 93  Request to revoke suspension"@en-AU ;
    dct:isPartOf C2020A00012:123 ;
    dct:isReferencedBy C2020A00012: ;
    rdfs:comment "93  Request to revoke suspension - Abrievated Graph Key: I125"@en-AU ;
    skos:definition "93  Request to revoke suspension"@en-AU ;
    skos:narrower C2020A00012:123 ;
    skos:prefLabel "Item I125"@en-AU ;
    dcat:accessURL <https://www.legislation.gov.au/C2020A00012/2024-07-10/2024-07-10/text/original/epub/OEBPS/document_1/document_1.html#_Toc172118817> ;
    dcat:landingPage "https://www.legislation.gov.au/C2020A00012/2024-07-10/2024-07-10/text/original/epub/OEBPS/document_1/document_1.html#_Toc172118817"^^xsd:anyURI ;
    dcat:theme legcons:Item .

C2020A00012:127 a legcons:Item,
        owl:Class,
        dcat:Resource ;
    rdfs:label "Item - I127 94  Grounds for suspensiongeneral"@en-AU ;
    dct:isPartOf C2020A00012:126 ;
    dct:isReferencedBy C2020A00012: ;
    rdfs:comment "94  Grounds for suspensiongeneral - Abrievated Graph Key: I127"@en-AU ;
    skos:definition "94  Grounds for suspensiongeneral"@en-AU ;
    skos:narrower C2020A00012:126 ;
    skos:prefLabel "Item I127"@en-AU ;
    dcat:accessURL <https://www.legislation.gov.au/C2020A00012/2024-07-10/2024-07-10/text/original/epub/OEBPS/document_1/document_1.html#_Toc172118819> ;
    dcat:landingPage "https://www.legislation.gov.au/C2020A00012/2024-07-10/2024-07-10/text/original/epub/OEBPS/document_1/document_1.html#_Toc172118819"^^xsd:anyURI ;
    dcat:theme legcons:Item .

C2020A00012:128 a legcons:Item,
        owl:Class,
        dcat:Resource ;
    rdfs:label "Item - I128 95  Grounds for suspensionoverdue relevant Commonwealth liability"@en-AU ;
    dct:isPartOf C2020A00012:126 ;
    dct:isReferencedBy C2020A00012: ;
    rdfs:comment "95  Grounds for suspensionoverdue relevant Commonwealth liability - Abrievated Graph Key: I128"@en-AU ;
    skos:definition "95  Grounds for suspensionoverdue relevant Commonwealth liability"@en-AU ;
    skos:narrower C2020A00012:126 ;
    skos:prefLabel "Item I128"@en-AU ;
    dcat:accessURL <https://www.legislation.gov.au/C2020A00012/2024-07-10/2024-07-10/text/original/epub/OEBPS/document_1/document_1.html#_Toc172118820> ;
    dcat:landingPage "https://www.legislation.gov.au/C2020A00012/2024-07-10/2024-07-10/text/original/epub/OEBPS/document_1/document_1.html#_Toc172118820"^^xsd:anyURI ;
    dcat:theme legcons:Item .

C2020A00012:129 a legcons:Item,
        owl:Class,
        dcat:Resource ;
    rdfs:label "Item - I129 96  Notice of suspension"@en-AU ;
    dct:isPartOf C2020A00012:126 ;
    dct:isReferencedBy C2020A00012: ;
    rdfs:comment "96  Notice of suspension - Abrievated Graph Key: I129"@en-AU ;
    skos:definition "96  Notice of suspension"@en-AU ;
    skos:narrower C2020A00012:126 ;
    skos:prefLabel "Item I129"@en-AU ;
    dcat:accessURL <https://www.legislation.gov.au/C2020A00012/2024-07-10/2024-07-10/text/original/epub/OEBPS/document_1/document_1.html#_Toc172118821> ;
    dcat:landingPage "https://www.legislation.gov.au/C2020A00012/2024-07-10/2024-07-10/text/original/epub/OEBPS/document_1/document_1.html#_Toc172118821"^^xsd:anyURI ;
    dcat:theme legcons:Item .

C2020A00012:13 a legcons:Item,
        owl:Class,
        dcat:Resource ;
    rdfs:label "Item - I13 11  Concurrent operation of State and Territory laws"@en-AU ;
    dct:isPartOf C2020A00012:1 ;
    dct:isReferencedBy C2020A00012: ;
    rdfs:comment "11  Concurrent operation of State and Territory laws - Abrievated Graph Key: I13"@en-AU ;
    skos:definition "11  Concurrent operation of State and Territory laws"@en-AU ;
    skos:narrower C2020A00012:1 ;
    skos:prefLabel "Item I13"@en-AU ;
    dcat:accessURL <https://www.legislation.gov.au/C2020A00012/2024-07-10/2024-07-10/text/original/epub/OEBPS/document_1/document_1.html#_Toc172118705> ;
    dcat:landingPage "https://www.legislation.gov.au/C2020A00012/2024-07-10/2024-07-10/text/original/epub/OEBPS/document_1/document_1.html#_Toc172118705"^^xsd:anyURI ;
    dcat:theme legcons:Item .

C2020A00012:130 a legcons:Item,
        owl:Class,
        dcat:Resource ;
    rdfs:label "Item - I130 97  Period of suspension"@en-AU ;
    dct:isPartOf C2020A00012:126 ;
    dct:isReferencedBy C2020A00012: ;
    rdfs:comment "97  Period of suspension - Abrievated Graph Key: I130"@en-AU ;
    skos:definition "97  Period of suspension"@en-AU ;
    skos:narrower C2020A00012:126 ;
    skos:prefLabel "Item I130"@en-AU ;
    dcat:accessURL <https://www.legislation.gov.au/C2020A00012/2024-07-10/2024-07-10/text/original/epub/OEBPS/document_1/document_1.html#_Toc172118822> ;
    dcat:landingPage "https://www.legislation.gov.au/C2020A00012/2024-07-10/2024-07-10/text/original/epub/OEBPS/document_1/document_1.html#_Toc172118822"^^xsd:anyURI ;
    dcat:theme legcons:Item .

C2020A00012:131 a legcons:Item,
        owl:Class,
        dcat:Resource ;
    rdfs:label "Item - I131 98  Revocation of suspension"@en-AU ;
    dct:isPartOf C2020A00012:126 ;
    dct:isReferencedBy C2020A00012: ;
    rdfs:comment "98  Revocation of suspension - Abrievated Graph Key: I131"@en-AU ;
    skos:definition "98  Revocation of suspension"@en-AU ;
    skos:narrower C2020A00012:126 ;
    skos:prefLabel "Item I131"@en-AU ;
    dcat:accessURL <https://www.legislation.gov.au/C2020A00012/2024-07-10/2024-07-10/text/original/epub/OEBPS/document_1/document_1.html#_Toc172118823> ;
    dcat:landingPage "https://www.legislation.gov.au/C2020A00012/2024-07-10/2024-07-10/text/original/epub/OEBPS/document_1/document_1.html#_Toc172118823"^^xsd:anyURI ;
    dcat:theme legcons:Item .

C2020A00012:133 a legcons:Item,
        owl:Class,
        dcat:Resource ;
    rdfs:label "Item - I133 99  Effect of suspension"@en-AU ;
    dct:isPartOf C2020A00012:132 ;
    dct:isReferencedBy C2020A00012: ;
    rdfs:comment "99  Effect of suspension - Abrievated Graph Key: I133"@en-AU ;
    skos:definition "99  Effect of suspension"@en-AU ;
    skos:narrower C2020A00012:132 ;
    skos:prefLabel "Item I133"@en-AU ;
    dcat:accessURL <https://www.legislation.gov.au/C2020A00012/2024-07-10/2024-07-10/text/original/epub/OEBPS/document_1/document_1.html#_Toc172118825> ;
    dcat:landingPage "https://www.legislation.gov.au/C2020A00012/2024-07-10/2024-07-10/text/original/epub/OEBPS/document_1/document_1.html#_Toc172118825"^^xsd:anyURI ;
    dcat:theme legcons:Item .

C2020A00012:134 a legcons:Item,
        owl:Class,
        dcat:Resource ;
    rdfs:label "Item - I134 100  Export operations must not be carried out while accreditation suspended"@en-AU ;
    dct:isPartOf C2020A00012:132 ;
    dct:isReferencedBy C2020A00012: ;
    rdfs:comment "100  Export operations must not be carried out while accreditation suspended - Abrievated Graph Key: I134"@en-AU ;
    skos:definition "100  Export operations must not be carried out while accreditation suspended"@en-AU ;
    skos:narrower C2020A00012:132 ;
    skos:prefLabel "Item I134"@en-AU ;
    dcat:accessURL <https://www.legislation.gov.au/C2020A00012/2024-07-10/2024-07-10/text/original/epub/OEBPS/document_1/document_1.html#_Toc172118826> ;
    dcat:landingPage "https://www.legislation.gov.au/C2020A00012/2024-07-10/2024-07-10/text/original/epub/OEBPS/document_1/document_1.html#_Toc172118826"^^xsd:anyURI ;
    dcat:theme legcons:Item .

C2020A00012:137 a legcons:Item,
        owl:Class,
        dcat:Resource ;
    rdfs:label "Item - I137 101  Manager may request revocation"@en-AU ;
    dct:isPartOf C2020A00012:136 ;
    dct:isReferencedBy C2020A00012: ;
    rdfs:comment "101  Manager may request revocation - Abrievated Graph Key: I137"@en-AU ;
    skos:definition "101  Manager may request revocation"@en-AU ;
    skos:narrower C2020A00012:136 ;
    skos:prefLabel "Item I137"@en-AU ;
    dcat:accessURL <https://www.legislation.gov.au/C2020A00012/2024-07-10/2024-07-10/text/original/epub/OEBPS/document_1/document_1.html#_Toc172118829> ;
    dcat:landingPage "https://www.legislation.gov.au/C2020A00012/2024-07-10/2024-07-10/text/original/epub/OEBPS/document_1/document_1.html#_Toc172118829"^^xsd:anyURI ;
    dcat:theme legcons:Item .

C2020A00012:139 a legcons:Item,
        owl:Class,
        dcat:Resource ;
    rdfs:label "Item - I139 102  Grounds for revocationgeneral"@en-AU ;
    dct:isPartOf C2020A00012:138 ;
    dct:isReferencedBy C2020A00012: ;
    rdfs:comment "102  Grounds for revocationgeneral - Abrievated Graph Key: I139"@en-AU ;
    skos:definition "102  Grounds for revocationgeneral"@en-AU ;
    skos:narrower C2020A00012:138 ;
    skos:prefLabel "Item I139"@en-AU ;
    dcat:accessURL <https://www.legislation.gov.au/C2020A00012/2024-07-10/2024-07-10/text/original/epub/OEBPS/document_1/document_1.html#_Toc172118831> ;
    dcat:landingPage "https://www.legislation.gov.au/C2020A00012/2024-07-10/2024-07-10/text/original/epub/OEBPS/document_1/document_1.html#_Toc172118831"^^xsd:anyURI ;
    dcat:theme legcons:Item .

C2020A00012:14 a legcons:Part,
        owl:Class,
        dcat:Resource ;
    rdfs:label "Part - P14 Part 2 Interpretation"@en-AU ;
    dct:isPartOf C2020A00012:1 ;
    dct:isReferencedBy C2020A00012: ;
    rdfs:comment "Part 2 Interpretation - Abrievated Graph Key: P14"@en-AU ;
    skos:definition "Part 2 Interpretation"@en-AU ;
    skos:narrower C2020A00012:1 ;
    skos:prefLabel "Part P14"@en-AU ;
    dcat:accessURL <https://www.legislation.gov.au/C2020A00012/2024-07-10/2024-07-10/text/original/epub/OEBPS/document_1/document_1.html#_Toc172118706> ;
    dcat:landingPage "https://www.legislation.gov.au/C2020A00012/2024-07-10/2024-07-10/text/original/epub/OEBPS/document_1/document_1.html#_Toc172118706"^^xsd:anyURI ;
    dcat:theme legcons:Part .

C2020A00012:140 a legcons:Item,
        owl:Class,
        dcat:Resource ;
    rdfs:label "Item - I140 103  Grounds for revocationoverdue relevant Commonwealth liability"@en-AU ;
    dct:isPartOf C2020A00012:138 ;
    dct:isReferencedBy C2020A00012: ;
    rdfs:comment "103  Grounds for revocationoverdue relevant Commonwealth liability - Abrievated Graph Key: I140"@en-AU ;
    skos:definition "103  Grounds for revocationoverdue relevant Commonwealth liability"@en-AU ;
    skos:narrower C2020A00012:138 ;
    skos:prefLabel "Item I140"@en-AU ;
    dcat:accessURL <https://www.legislation.gov.au/C2020A00012/2024-07-10/2024-07-10/text/original/epub/OEBPS/document_1/document_1.html#_Toc172118832> ;
    dcat:landingPage "https://www.legislation.gov.au/C2020A00012/2024-07-10/2024-07-10/text/original/epub/OEBPS/document_1/document_1.html#_Toc172118832"^^xsd:anyURI ;
    dcat:theme legcons:Item .

C2020A00012:141 a legcons:Item,
        owl:Class,
        dcat:Resource ;
    rdfs:label "Item - I141 104  Notice of revocation"@en-AU ;
    dct:isPartOf C2020A00012:138 ;
    dct:isReferencedBy C2020A00012: ;
    rdfs:comment "104  Notice of revocation - Abrievated Graph Key: I141"@en-AU ;
    skos:definition "104  Notice of revocation"@en-AU ;
    skos:narrower C2020A00012:138 ;
    skos:prefLabel "Item I141"@en-AU ;
    dcat:accessURL <https://www.legislation.gov.au/C2020A00012/2024-07-10/2024-07-10/text/original/epub/OEBPS/document_1/document_1.html#_Toc172118833> ;
    dcat:landingPage "https://www.legislation.gov.au/C2020A00012/2024-07-10/2024-07-10/text/original/epub/OEBPS/document_1/document_1.html#_Toc172118833"^^xsd:anyURI ;
    dcat:theme legcons:Item .

C2020A00012:143 a legcons:Item,
        owl:Class,
        dcat:Resource ;
    rdfs:label "Item - I143 105  Secretary may require action to be taken after accreditation revoked"@en-AU ;
    dct:isPartOf C2020A00012:142 ;
    dct:isReferencedBy C2020A00012: ;
    rdfs:comment "105  Secretary may require action to be taken after accreditation revoked - Abrievated Graph Key: I143"@en-AU ;
    skos:definition "105  Secretary may require action to be taken after accreditation revoked"@en-AU ;
    skos:narrower C2020A00012:142 ;
    skos:prefLabel "Item I143"@en-AU ;
    dcat:accessURL <https://www.legislation.gov.au/C2020A00012/2024-07-10/2024-07-10/text/original/epub/OEBPS/document_1/document_1.html#_Toc172118835> ;
    dcat:landingPage "https://www.legislation.gov.au/C2020A00012/2024-07-10/2024-07-10/text/original/epub/OEBPS/document_1/document_1.html#_Toc172118835"^^xsd:anyURI ;
    dcat:theme legcons:Item .

C2020A00012:145 a legcons:Item,
        owl:Class,
        dcat:Resource ;
    rdfs:label "Item - I145 106  Conditions of accreditation must not be contravened"@en-AU ;
    dct:isPartOf C2020A00012:144 ;
    dct:isReferencedBy C2020A00012: ;
    rdfs:comment "106  Conditions of accreditation must not be contravened - Abrievated Graph Key: I145"@en-AU ;
    skos:definition "106  Conditions of accreditation must not be contravened"@en-AU ;
    skos:narrower C2020A00012:144 ;
    skos:prefLabel "Item I145"@en-AU ;
    dcat:accessURL <https://www.legislation.gov.au/C2020A00012/2024-07-10/2024-07-10/text/original/epub/OEBPS/document_1/document_1.html#_Toc172118837> ;
    dcat:landingPage "https://www.legislation.gov.au/C2020A00012/2024-07-10/2024-07-10/text/original/epub/OEBPS/document_1/document_1.html#_Toc172118837"^^xsd:anyURI ;
    dcat:theme legcons:Item .

C2020A00012:146 a legcons:Item,
        owl:Class,
        dcat:Resource ;
    rdfs:label "Item - I146 107  Additional or corrected information in relation to application for accreditation etc"@en-AU ;
    dct:isPartOf C2020A00012:144 ;
    dct:isReferencedBy C2020A00012: ;
    rdfs:comment "107  Additional or corrected information in relation to application for accreditation etc - Abrievated Graph Key: I146"@en-AU ;
    skos:definition "107  Additional or corrected information in relation to application for accreditation etc"@en-AU ;
    skos:narrower C2020A00012:144 ;
    skos:prefLabel "Item I146"@en-AU ;
    dcat:accessURL <https://www.legislation.gov.au/C2020A00012/2024-07-10/2024-07-10/text/original/epub/OEBPS/document_1/document_1.html#_Toc172118838> ;
    dcat:landingPage "https://www.legislation.gov.au/C2020A00012/2024-07-10/2024-07-10/text/original/epub/OEBPS/document_1/document_1.html#_Toc172118838"^^xsd:anyURI ;
    dcat:theme legcons:Item .

C2020A00012:147 a legcons:Item,
        owl:Class,
        dcat:Resource ;
    rdfs:label "Item - I147 108  Notice of event or change in circumstances"@en-AU ;
    dct:isPartOf C2020A00012:144 ;
    dct:isReferencedBy C2020A00012: ;
    rdfs:comment "108  Notice of event or change in circumstances - Abrievated Graph Key: I147"@en-AU ;
    skos:definition "108  Notice of event or change in circumstances"@en-AU ;
    skos:narrower C2020A00012:144 ;
    skos:prefLabel "Item I147"@en-AU ;
    dcat:accessURL <https://www.legislation.gov.au/C2020A00012/2024-07-10/2024-07-10/text/original/epub/OEBPS/document_1/document_1.html#_Toc172118839> ;
    dcat:landingPage "https://www.legislation.gov.au/C2020A00012/2024-07-10/2024-07-10/text/original/epub/OEBPS/document_1/document_1.html#_Toc172118839"^^xsd:anyURI ;
    dcat:theme legcons:Item .

C2020A00012:148 a legcons:Item,
        owl:Class,
        dcat:Resource ;
    rdfs:label "Item - I148 109  Notice of person ceasing to be manager of accredited property"@en-AU ;
    dct:isPartOf C2020A00012:144 ;
    dct:isReferencedBy C2020A00012: ;
    rdfs:comment "109  Notice of person ceasing to be manager of accredited property - Abrievated Graph Key: I148"@en-AU ;
    skos:definition "109  Notice of person ceasing to be manager of accredited property"@en-AU ;
    skos:narrower C2020A00012:144 ;
    skos:prefLabel "Item I148"@en-AU ;
    dcat:accessURL <https://www.legislation.gov.au/C2020A00012/2024-07-10/2024-07-10/text/original/epub/OEBPS/document_1/document_1.html#_Toc172118840> ;
    dcat:landingPage "https://www.legislation.gov.au/C2020A00012/2024-07-10/2024-07-10/text/original/epub/OEBPS/document_1/document_1.html#_Toc172118840"^^xsd:anyURI ;
    dcat:theme legcons:Item .

C2020A00012:15 a legcons:Division,
        owl:Class,
        dcat:Resource ;
    rdfs:label "Division - D15 Division 1 Definitions"@en-AU ;
    dct:isPartOf C2020A00012:1 ;
    dct:isReferencedBy C2020A00012: ;
    rdfs:comment "Division 1 Definitions - Abrievated Graph Key: D15"@en-AU ;
    skos:definition "Division 1 Definitions"@en-AU ;
    skos:narrower C2020A00012:1 ;
    skos:prefLabel "Division D15"@en-AU ;
    dcat:accessURL <https://www.legislation.gov.au/C2020A00012/2024-07-10/2024-07-10/text/original/epub/OEBPS/document_1/document_1.html#_Toc172118707> ;
    dcat:landingPage "https://www.legislation.gov.au/C2020A00012/2024-07-10/2024-07-10/text/original/epub/OEBPS/document_1/document_1.html#_Toc172118707"^^xsd:anyURI ;
    dcat:theme legcons:Division .

C2020A00012:151 a legcons:Item,
        owl:Class,
        dcat:Resource ;
    rdfs:label "Item - I151 110  Simplified outline of this Chapter"@en-AU ;
    dct:isPartOf C2020A00012:150 ;
    dct:isReferencedBy C2020A00012: ;
    rdfs:comment "110  Simplified outline of this Chapter - Abrievated Graph Key: I151"@en-AU ;
    skos:definition "110  Simplified outline of this Chapter"@en-AU ;
    skos:narrower C2020A00012:150 ;
    skos:prefLabel "Item I151"@en-AU ;
    dcat:accessURL <https://www.legislation.gov.au/C2020A00012/2024-07-10/2024-07-10/text/original/epub/OEBPS/document_1/document_1.html#_Toc172118843> ;
    dcat:landingPage "https://www.legislation.gov.au/C2020A00012/2024-07-10/2024-07-10/text/original/epub/OEBPS/document_1/document_1.html#_Toc172118843"^^xsd:anyURI ;
    dcat:theme legcons:Item .

C2020A00012:153 a legcons:Item,
        owl:Class,
        dcat:Resource ;
    rdfs:label "Item - I153 111  Application for registration of establishment"@en-AU ;
    dct:isPartOf C2020A00012:152 ;
    dct:isReferencedBy C2020A00012: ;
    rdfs:comment "111  Application for registration of establishment - Abrievated Graph Key: I153"@en-AU ;
    skos:definition "111  Application for registration of establishment"@en-AU ;
    skos:narrower C2020A00012:152 ;
    skos:prefLabel "Item I153"@en-AU ;
    dcat:accessURL <https://www.legislation.gov.au/C2020A00012/2024-07-10/2024-07-10/text/original/epub/OEBPS/document_1/document_1.html#_Toc172118845> ;
    dcat:landingPage "https://www.legislation.gov.au/C2020A00012/2024-07-10/2024-07-10/text/original/epub/OEBPS/document_1/document_1.html#_Toc172118845"^^xsd:anyURI ;
    dcat:theme legcons:Item .

C2020A00012:154 a legcons:Item,
        owl:Class,
        dcat:Resource ;
    rdfs:label "Item - I154 112  Secretary must decide whether to register establishment"@en-AU ;
    dct:isPartOf C2020A00012:152 ;
    dct:isReferencedBy C2020A00012: ;
    rdfs:comment "112  Secretary must decide whether to register establishment - Abrievated Graph Key: I154"@en-AU ;
    skos:definition "112  Secretary must decide whether to register establishment"@en-AU ;
    skos:narrower C2020A00012:152 ;
    skos:prefLabel "Item I154"@en-AU ;
    dcat:accessURL <https://www.legislation.gov.au/C2020A00012/2024-07-10/2024-07-10/text/original/epub/OEBPS/document_1/document_1.html#_Toc172118846> ;
    dcat:landingPage "https://www.legislation.gov.au/C2020A00012/2024-07-10/2024-07-10/text/original/epub/OEBPS/document_1/document_1.html#_Toc172118846"^^xsd:anyURI ;
    dcat:theme legcons:Item .

C2020A00012:155 a legcons:Item,
        owl:Class,
        dcat:Resource ;
    rdfs:label "Item - I155 113  Conditions of registration"@en-AU ;
    dct:isPartOf C2020A00012:152 ;
    dct:isReferencedBy C2020A00012: ;
    rdfs:comment "113  Conditions of registration - Abrievated Graph Key: I155"@en-AU ;
    skos:definition "113  Conditions of registration"@en-AU ;
    skos:narrower C2020A00012:152 ;
    skos:prefLabel "Item I155"@en-AU ;
    dcat:accessURL <https://www.legislation.gov.au/C2020A00012/2024-07-10/2024-07-10/text/original/epub/OEBPS/document_1/document_1.html#_Toc172118847> ;
    dcat:landingPage "https://www.legislation.gov.au/C2020A00012/2024-07-10/2024-07-10/text/original/epub/OEBPS/document_1/document_1.html#_Toc172118847"^^xsd:anyURI ;
    dcat:theme legcons:Item .

C2020A00012:156 a legcons:Item,
        owl:Class,
        dcat:Resource ;
    rdfs:label "Item - I156 114  Notice of decision and certificate of registration"@en-AU ;
    dct:isPartOf C2020A00012:152 ;
    dct:isReferencedBy C2020A00012: ;
    rdfs:comment "114  Notice of decision and certificate of registration - Abrievated Graph Key: I156"@en-AU ;
    skos:definition "114  Notice of decision and certificate of registration"@en-AU ;
    skos:narrower C2020A00012:152 ;
    skos:prefLabel "Item I156"@en-AU ;
    dcat:accessURL <https://www.legislation.gov.au/C2020A00012/2024-07-10/2024-07-10/text/original/epub/OEBPS/document_1/document_1.html#_Toc172118848> ;
    dcat:landingPage "https://www.legislation.gov.au/C2020A00012/2024-07-10/2024-07-10/text/original/epub/OEBPS/document_1/document_1.html#_Toc172118848"^^xsd:anyURI ;
    dcat:theme legcons:Item .

C2020A00012:157 a legcons:Item,
        owl:Class,
        dcat:Resource ;
    rdfs:label "Item - I157 115  Period of effect of registration"@en-AU ;
    dct:isPartOf C2020A00012:152 ;
    dct:isReferencedBy C2020A00012: ;
    rdfs:comment "115  Period of effect of registration - Abrievated Graph Key: I157"@en-AU ;
    skos:definition "115  Period of effect of registration"@en-AU ;
    skos:narrower C2020A00012:152 ;
    skos:prefLabel "Item I157"@en-AU ;
    dcat:accessURL <https://www.legislation.gov.au/C2020A00012/2024-07-10/2024-07-10/text/original/epub/OEBPS/document_1/document_1.html#_Toc172118849> ;
    dcat:landingPage "https://www.legislation.gov.au/C2020A00012/2024-07-10/2024-07-10/text/original/epub/OEBPS/document_1/document_1.html#_Toc172118849"^^xsd:anyURI ;
    dcat:theme legcons:Item .

C2020A00012:159 a legcons:Item,
        owl:Class,
        dcat:Resource ;
    rdfs:label "Item - I159 116  Application to renew registration of establishment"@en-AU ;
    dct:isPartOf C2020A00012:158 ;
    dct:isReferencedBy C2020A00012: ;
    rdfs:comment "116  Application to renew registration of establishment - Abrievated Graph Key: I159"@en-AU ;
    skos:definition "116  Application to renew registration of establishment"@en-AU ;
    skos:narrower C2020A00012:158 ;
    skos:prefLabel "Item I159"@en-AU ;
    dcat:accessURL <https://www.legislation.gov.au/C2020A00012/2024-07-10/2024-07-10/text/original/epub/OEBPS/document_1/document_1.html#_Toc172118851> ;
    dcat:landingPage "https://www.legislation.gov.au/C2020A00012/2024-07-10/2024-07-10/text/original/epub/OEBPS/document_1/document_1.html#_Toc172118851"^^xsd:anyURI ;
    dcat:theme legcons:Item .

C2020A00012:16 a legcons:Item,
        owl:Class,
        dcat:Resource ;
    rdfs:label "Item - I16 12  Definitions"@en-AU ;
    dct:isPartOf C2020A00012:1 ;
    dct:isReferencedBy C2020A00012: ;
    rdfs:comment "12  Definitions - Abrievated Graph Key: I16"@en-AU ;
    skos:definition "12  Definitions"@en-AU ;
    skos:narrower C2020A00012:1 ;
    skos:prefLabel "Item I16"@en-AU ;
    dcat:accessURL <https://www.legislation.gov.au/C2020A00012/2024-07-10/2024-07-10/text/original/epub/OEBPS/document_1/document_1.html#_Toc172118708> ;
    dcat:landingPage "https://www.legislation.gov.au/C2020A00012/2024-07-10/2024-07-10/text/original/epub/OEBPS/document_1/document_1.html#_Toc172118708"^^xsd:anyURI ;
    dcat:theme legcons:Item .

C2020A00012:160 a legcons:Item,
        owl:Class,
        dcat:Resource ;
    rdfs:label "Item - I160 117  Secretary must decide whether to renew registration"@en-AU ;
    dct:isPartOf C2020A00012:158 ;
    dct:isReferencedBy C2020A00012: ;
    rdfs:comment "117  Secretary must decide whether to renew registration - Abrievated Graph Key: I160"@en-AU ;
    skos:definition "117  Secretary must decide whether to renew registration"@en-AU ;
    skos:narrower C2020A00012:158 ;
    skos:prefLabel "Item I160"@en-AU ;
    dcat:accessURL <https://www.legislation.gov.au/C2020A00012/2024-07-10/2024-07-10/text/original/epub/OEBPS/document_1/document_1.html#_Toc172118852> ;
    dcat:landingPage "https://www.legislation.gov.au/C2020A00012/2024-07-10/2024-07-10/text/original/epub/OEBPS/document_1/document_1.html#_Toc172118852"^^xsd:anyURI ;
    dcat:theme legcons:Item .

C2020A00012:161 a legcons:Item,
        owl:Class,
        dcat:Resource ;
    rdfs:label "Item - I161 118  Conditions of renewed registration"@en-AU ;
    dct:isPartOf C2020A00012:158 ;
    dct:isReferencedBy C2020A00012: ;
    rdfs:comment "118  Conditions of renewed registration - Abrievated Graph Key: I161"@en-AU ;
    skos:definition "118  Conditions of renewed registration"@en-AU ;
    skos:narrower C2020A00012:158 ;
    skos:prefLabel "Item I161"@en-AU ;
    dcat:accessURL <https://www.legislation.gov.au/C2020A00012/2024-07-10/2024-07-10/text/original/epub/OEBPS/document_1/document_1.html#_Toc172118853> ;
    dcat:landingPage "https://www.legislation.gov.au/C2020A00012/2024-07-10/2024-07-10/text/original/epub/OEBPS/document_1/document_1.html#_Toc172118853"^^xsd:anyURI ;
    dcat:theme legcons:Item .

C2020A00012:162 a legcons:Item,
        owl:Class,
        dcat:Resource ;
    rdfs:label "Item - I162 119  Notice of decision and certificate of registration"@en-AU ;
    dct:isPartOf C2020A00012:158 ;
    dct:isReferencedBy C2020A00012: ;
    rdfs:comment "119  Notice of decision and certificate of registration - Abrievated Graph Key: I162"@en-AU ;
    skos:definition "119  Notice of decision and certificate of registration"@en-AU ;
    skos:narrower C2020A00012:158 ;
    skos:prefLabel "Item I162"@en-AU ;
    dcat:accessURL <https://www.legislation.gov.au/C2020A00012/2024-07-10/2024-07-10/text/original/epub/OEBPS/document_1/document_1.html#_Toc172118854> ;
    dcat:landingPage "https://www.legislation.gov.au/C2020A00012/2024-07-10/2024-07-10/text/original/epub/OEBPS/document_1/document_1.html#_Toc172118854"^^xsd:anyURI ;
    dcat:theme legcons:Item .

C2020A00012:165 a legcons:Item,
        owl:Class,
        dcat:Resource ;
    rdfs:label "Item - I165 120  Application by occupier for variation of registration or approval of alteration of establishment"@en-AU ;
    dct:isPartOf C2020A00012:164 ;
    dct:isReferencedBy C2020A00012: ;
    rdfs:comment "120  Application by occupier for variation of registration or approval of alteration of establishment - Abrievated Graph Key: I165"@en-AU ;
    skos:definition "120  Application by occupier for variation of registration or approval of alteration of establishment"@en-AU ;
    skos:narrower C2020A00012:164 ;
    skos:prefLabel "Item I165"@en-AU ;
    dcat:accessURL <https://www.legislation.gov.au/C2020A00012/2024-07-10/2024-07-10/text/original/epub/OEBPS/document_1/document_1.html#_Toc172118857> ;
    dcat:landingPage "https://www.legislation.gov.au/C2020A00012/2024-07-10/2024-07-10/text/original/epub/OEBPS/document_1/document_1.html#_Toc172118857"^^xsd:anyURI ;
    dcat:theme legcons:Item .

C2020A00012:166 a legcons:Item,
        owl:Class,
        dcat:Resource ;
    rdfs:label "Item - I166 121  Notice of variation or approval of alteration"@en-AU ;
    dct:isPartOf C2020A00012:164 ;
    dct:isReferencedBy C2020A00012: ;
    rdfs:comment "121  Notice of variation or approval of alteration - Abrievated Graph Key: I166"@en-AU ;
    skos:definition "121  Notice of variation or approval of alteration"@en-AU ;
    skos:narrower C2020A00012:164 ;
    skos:prefLabel "Item I166"@en-AU ;
    dcat:accessURL <https://www.legislation.gov.au/C2020A00012/2024-07-10/2024-07-10/text/original/epub/OEBPS/document_1/document_1.html#_Toc172118858> ;
    dcat:landingPage "https://www.legislation.gov.au/C2020A00012/2024-07-10/2024-07-10/text/original/epub/OEBPS/document_1/document_1.html#_Toc172118858"^^xsd:anyURI ;
    dcat:theme legcons:Item .

C2020A00012:167 a legcons:Item,
        owl:Class,
        dcat:Resource ;
    rdfs:label "Item - I167 122  Certain alterations of registered establishment must not be made unless approved etc"@en-AU ;
    dct:isPartOf C2020A00012:164 ;
    dct:isReferencedBy C2020A00012: ;
    rdfs:comment "122  Certain alterations of registered establishment must not be made unless approved etc - Abrievated Graph Key: I167"@en-AU ;
    skos:definition "122  Certain alterations of registered establishment must not be made unless approved etc"@en-AU ;
    skos:narrower C2020A00012:164 ;
    skos:prefLabel "Item I167"@en-AU ;
    dcat:accessURL <https://www.legislation.gov.au/C2020A00012/2024-07-10/2024-07-10/text/original/epub/OEBPS/document_1/document_1.html#_Toc172118859> ;
    dcat:landingPage "https://www.legislation.gov.au/C2020A00012/2024-07-10/2024-07-10/text/original/epub/OEBPS/document_1/document_1.html#_Toc172118859"^^xsd:anyURI ;
    dcat:theme legcons:Item .

C2020A00012:169 a legcons:Item,
        owl:Class,
        dcat:Resource ;
    rdfs:label "Item - I169 123  Secretary may make variations in relation to registration"@en-AU ;
    dct:isPartOf C2020A00012:168 ;
    dct:isReferencedBy C2020A00012: ;
    rdfs:comment "123  Secretary may make variations in relation to registration - Abrievated Graph Key: I169"@en-AU ;
    skos:definition "123  Secretary may make variations in relation to registration"@en-AU ;
    skos:narrower C2020A00012:168 ;
    skos:prefLabel "Item I169"@en-AU ;
    dcat:accessURL <https://www.legislation.gov.au/C2020A00012/2024-07-10/2024-07-10/text/original/epub/OEBPS/document_1/document_1.html#_Toc172118861> ;
    dcat:landingPage "https://www.legislation.gov.au/C2020A00012/2024-07-10/2024-07-10/text/original/epub/OEBPS/document_1/document_1.html#_Toc172118861"^^xsd:anyURI ;
    dcat:theme legcons:Item .

C2020A00012:17 a legcons:Item,
        owl:Class,
        dcat:Resource ;
    rdfs:label "Item - I17 13  Meaning of associate"@en-AU ;
    dct:isPartOf C2020A00012:1 ;
    dct:isReferencedBy C2020A00012: ;
    rdfs:comment "13  Meaning of associate - Abrievated Graph Key: I17"@en-AU ;
    skos:definition "13  Meaning of associate"@en-AU ;
    skos:narrower C2020A00012:1 ;
    skos:prefLabel "Item I17"@en-AU ;
    dcat:accessURL <https://www.legislation.gov.au/C2020A00012/2024-07-10/2024-07-10/text/original/epub/OEBPS/document_1/document_1.html#_Toc172118709> ;
    dcat:landingPage "https://www.legislation.gov.au/C2020A00012/2024-07-10/2024-07-10/text/original/epub/OEBPS/document_1/document_1.html#_Toc172118709"^^xsd:anyURI ;
    dcat:theme legcons:Item .

C2020A00012:170 a legcons:Item,
        owl:Class,
        dcat:Resource ;
    rdfs:label "Item - I170 124  Notice of variation"@en-AU ;
    dct:isPartOf C2020A00012:168 ;
    dct:isReferencedBy C2020A00012: ;
    rdfs:comment "124  Notice of variation - Abrievated Graph Key: I170"@en-AU ;
    skos:definition "124  Notice of variation"@en-AU ;
    skos:narrower C2020A00012:168 ;
    skos:prefLabel "Item I170"@en-AU ;
    dcat:accessURL <https://www.legislation.gov.au/C2020A00012/2024-07-10/2024-07-10/text/original/epub/OEBPS/document_1/document_1.html#_Toc172118862> ;
    dcat:landingPage "https://www.legislation.gov.au/C2020A00012/2024-07-10/2024-07-10/text/original/epub/OEBPS/document_1/document_1.html#_Toc172118862"^^xsd:anyURI ;
    dcat:theme legcons:Item .

C2020A00012:173 a legcons:Item,
        owl:Class,
        dcat:Resource ;
    rdfs:label "Item - I173 125  Occupier may request suspension"@en-AU ;
    dct:isPartOf C2020A00012:172 ;
    dct:isReferencedBy C2020A00012: ;
    rdfs:comment "125  Occupier may request suspension - Abrievated Graph Key: I173"@en-AU ;
    skos:definition "125  Occupier may request suspension"@en-AU ;
    skos:narrower C2020A00012:172 ;
    skos:prefLabel "Item I173"@en-AU ;
    dcat:accessURL <https://www.legislation.gov.au/C2020A00012/2024-07-10/2024-07-10/text/original/epub/OEBPS/document_1/document_1.html#_Toc172118865> ;
    dcat:landingPage "https://www.legislation.gov.au/C2020A00012/2024-07-10/2024-07-10/text/original/epub/OEBPS/document_1/document_1.html#_Toc172118865"^^xsd:anyURI ;
    dcat:theme legcons:Item .

C2020A00012:174 a legcons:Item,
        owl:Class,
        dcat:Resource ;
    rdfs:label "Item - I174 126  Request to revoke suspension"@en-AU ;
    dct:isPartOf C2020A00012:172 ;
    dct:isReferencedBy C2020A00012: ;
    rdfs:comment "126  Request to revoke suspension - Abrievated Graph Key: I174"@en-AU ;
    skos:definition "126  Request to revoke suspension"@en-AU ;
    skos:narrower C2020A00012:172 ;
    skos:prefLabel "Item I174"@en-AU ;
    dcat:accessURL <https://www.legislation.gov.au/C2020A00012/2024-07-10/2024-07-10/text/original/epub/OEBPS/document_1/document_1.html#_Toc172118866> ;
    dcat:landingPage "https://www.legislation.gov.au/C2020A00012/2024-07-10/2024-07-10/text/original/epub/OEBPS/document_1/document_1.html#_Toc172118866"^^xsd:anyURI ;
    dcat:theme legcons:Item .

C2020A00012:176 a legcons:Item,
        owl:Class,
        dcat:Resource ;
    rdfs:label "Item - I176 127  Grounds for suspensiongeneral"@en-AU ;
    dct:isPartOf C2020A00012:175 ;
    dct:isReferencedBy C2020A00012: ;
    rdfs:comment "127  Grounds for suspensiongeneral - Abrievated Graph Key: I176"@en-AU ;
    skos:definition "127  Grounds for suspensiongeneral"@en-AU ;
    skos:narrower C2020A00012:175 ;
    skos:prefLabel "Item I176"@en-AU ;
    dcat:accessURL <https://www.legislation.gov.au/C2020A00012/2024-07-10/2024-07-10/text/original/epub/OEBPS/document_1/document_1.html#_Toc172118868> ;
    dcat:landingPage "https://www.legislation.gov.au/C2020A00012/2024-07-10/2024-07-10/text/original/epub/OEBPS/document_1/document_1.html#_Toc172118868"^^xsd:anyURI ;
    dcat:theme legcons:Item .

C2020A00012:177 a legcons:Item,
        owl:Class,
        dcat:Resource ;
    rdfs:label "Item - I177 128  Grounds for suspensionoverdue relevant Commonwealth liability"@en-AU ;
    dct:isPartOf C2020A00012:175 ;
    dct:isReferencedBy C2020A00012: ;
    rdfs:comment "128  Grounds for suspensionoverdue relevant Commonwealth liability - Abrievated Graph Key: I177"@en-AU ;
    skos:definition "128  Grounds for suspensionoverdue relevant Commonwealth liability"@en-AU ;
    skos:narrower C2020A00012:175 ;
    skos:prefLabel "Item I177"@en-AU ;
    dcat:accessURL <https://www.legislation.gov.au/C2020A00012/2024-07-10/2024-07-10/text/original/epub/OEBPS/document_1/document_1.html#_Toc172118869> ;
    dcat:landingPage "https://www.legislation.gov.au/C2020A00012/2024-07-10/2024-07-10/text/original/epub/OEBPS/document_1/document_1.html#_Toc172118869"^^xsd:anyURI ;
    dcat:theme legcons:Item .

C2020A00012:178 a legcons:Item,
        owl:Class,
        dcat:Resource ;
    rdfs:label "Item - I178 129  Notice of suspension"@en-AU ;
    dct:isPartOf C2020A00012:175 ;
    dct:isReferencedBy C2020A00012: ;
    rdfs:comment "129  Notice of suspension - Abrievated Graph Key: I178"@en-AU ;
    skos:definition "129  Notice of suspension"@en-AU ;
    skos:narrower C2020A00012:175 ;
    skos:prefLabel "Item I178"@en-AU ;
    dcat:accessURL <https://www.legislation.gov.au/C2020A00012/2024-07-10/2024-07-10/text/original/epub/OEBPS/document_1/document_1.html#_Toc172118870> ;
    dcat:landingPage "https://www.legislation.gov.au/C2020A00012/2024-07-10/2024-07-10/text/original/epub/OEBPS/document_1/document_1.html#_Toc172118870"^^xsd:anyURI ;
    dcat:theme legcons:Item .

C2020A00012:179 a legcons:Item,
        owl:Class,
        dcat:Resource ;
    rdfs:label "Item - I179 130  Period of suspension"@en-AU ;
    dct:isPartOf C2020A00012:175 ;
    dct:isReferencedBy C2020A00012: ;
    rdfs:comment "130  Period of suspension - Abrievated Graph Key: I179"@en-AU ;
    skos:definition "130  Period of suspension"@en-AU ;
    skos:narrower C2020A00012:175 ;
    skos:prefLabel "Item I179"@en-AU ;
    dcat:accessURL <https://www.legislation.gov.au/C2020A00012/2024-07-10/2024-07-10/text/original/epub/OEBPS/document_1/document_1.html#_Toc172118871> ;
    dcat:landingPage "https://www.legislation.gov.au/C2020A00012/2024-07-10/2024-07-10/text/original/epub/OEBPS/document_1/document_1.html#_Toc172118871"^^xsd:anyURI ;
    dcat:theme legcons:Item .

C2020A00012:18 a legcons:Item,
        owl:Class,
        dcat:Resource ;
    rdfs:label "Item - I18 14  Meaning of Australian territory"@en-AU ;
    dct:isPartOf C2020A00012:1 ;
    dct:isReferencedBy C2020A00012: ;
    rdfs:comment "14  Meaning of Australian territory - Abrievated Graph Key: I18"@en-AU ;
    skos:definition "14  Meaning of Australian territory"@en-AU ;
    skos:narrower C2020A00012:1 ;
    skos:prefLabel "Item I18"@en-AU ;
    dcat:accessURL <https://www.legislation.gov.au/C2020A00012/2024-07-10/2024-07-10/text/original/epub/OEBPS/document_1/document_1.html#_Toc172118710> ;
    dcat:landingPage "https://www.legislation.gov.au/C2020A00012/2024-07-10/2024-07-10/text/original/epub/OEBPS/document_1/document_1.html#_Toc172118710"^^xsd:anyURI ;
    dcat:theme legcons:Item .

C2020A00012:180 a legcons:Item,
        owl:Class,
        dcat:Resource ;
    rdfs:label "Item - I180 131  Revocation of suspension"@en-AU ;
    dct:isPartOf C2020A00012:175 ;
    dct:isReferencedBy C2020A00012: ;
    rdfs:comment "131  Revocation of suspension - Abrievated Graph Key: I180"@en-AU ;
    skos:definition "131  Revocation of suspension"@en-AU ;
    skos:narrower C2020A00012:175 ;
    skos:prefLabel "Item I180"@en-AU ;
    dcat:accessURL <https://www.legislation.gov.au/C2020A00012/2024-07-10/2024-07-10/text/original/epub/OEBPS/document_1/document_1.html#_Toc172118872> ;
    dcat:landingPage "https://www.legislation.gov.au/C2020A00012/2024-07-10/2024-07-10/text/original/epub/OEBPS/document_1/document_1.html#_Toc172118872"^^xsd:anyURI ;
    dcat:theme legcons:Item .

C2020A00012:182 a legcons:Item,
        owl:Class,
        dcat:Resource ;
    rdfs:label "Item - I182 132  Direction to cease carrying out export operationsfailure to comply with conditions or requirements of this Act etc"@en-AU ;
    dct:isPartOf C2020A00012:181 ;
    dct:isReferencedBy C2020A00012: ;
    rdfs:comment "132  Direction to cease carrying out export operationsfailure to comply with conditions or requirements of this Act etc - Abrievated Graph Key: I182"@en-AU ;
    skos:definition "132  Direction to cease carrying out export operationsfailure to comply with conditions or requirements of this Act etc"@en-AU ;
    skos:narrower C2020A00012:181 ;
    skos:prefLabel "Item I182"@en-AU ;
    dcat:accessURL <https://www.legislation.gov.au/C2020A00012/2024-07-10/2024-07-10/text/original/epub/OEBPS/document_1/document_1.html#_Toc172118874> ;
    dcat:landingPage "https://www.legislation.gov.au/C2020A00012/2024-07-10/2024-07-10/text/original/epub/OEBPS/document_1/document_1.html#_Toc172118874"^^xsd:anyURI ;
    dcat:theme legcons:Item .

C2020A00012:183 a legcons:Item,
        owl:Class,
        dcat:Resource ;
    rdfs:label "Item - I183 133  Occupier must comply with direction"@en-AU ;
    dct:isPartOf C2020A00012:181 ;
    dct:isReferencedBy C2020A00012: ;
    rdfs:comment "133  Occupier must comply with direction - Abrievated Graph Key: I183"@en-AU ;
    skos:definition "133  Occupier must comply with direction"@en-AU ;
    skos:narrower C2020A00012:181 ;
    skos:prefLabel "Item I183"@en-AU ;
    dcat:accessURL <https://www.legislation.gov.au/C2020A00012/2024-07-10/2024-07-10/text/original/epub/OEBPS/document_1/document_1.html#_Toc172118875> ;
    dcat:landingPage "https://www.legislation.gov.au/C2020A00012/2024-07-10/2024-07-10/text/original/epub/OEBPS/document_1/document_1.html#_Toc172118875"^^xsd:anyURI ;
    dcat:theme legcons:Item .

C2020A00012:184 a legcons:Item,
        owl:Class,
        dcat:Resource ;
    rdfs:label "Item - I184 134  Revocation of direction"@en-AU ;
    dct:isPartOf C2020A00012:181 ;
    dct:isReferencedBy C2020A00012: ;
    rdfs:comment "134  Revocation of direction - Abrievated Graph Key: I184"@en-AU ;
    skos:definition "134  Revocation of direction"@en-AU ;
    skos:narrower C2020A00012:181 ;
    skos:prefLabel "Item I184"@en-AU ;
    dcat:accessURL <https://www.legislation.gov.au/C2020A00012/2024-07-10/2024-07-10/text/original/epub/OEBPS/document_1/document_1.html#_Toc172118876> ;
    dcat:landingPage "https://www.legislation.gov.au/C2020A00012/2024-07-10/2024-07-10/text/original/epub/OEBPS/document_1/document_1.html#_Toc172118876"^^xsd:anyURI ;
    dcat:theme legcons:Item .

C2020A00012:186 a legcons:Item,
        owl:Class,
        dcat:Resource ;
    rdfs:label "Item - I186 135  Effect of suspension"@en-AU ;
    dct:isPartOf C2020A00012:185 ;
    dct:isReferencedBy C2020A00012: ;
    rdfs:comment "135  Effect of suspension - Abrievated Graph Key: I186"@en-AU ;
    skos:definition "135  Effect of suspension"@en-AU ;
    skos:narrower C2020A00012:185 ;
    skos:prefLabel "Item I186"@en-AU ;
    dcat:accessURL <https://www.legislation.gov.au/C2020A00012/2024-07-10/2024-07-10/text/original/epub/OEBPS/document_1/document_1.html#_Toc172118878> ;
    dcat:landingPage "https://www.legislation.gov.au/C2020A00012/2024-07-10/2024-07-10/text/original/epub/OEBPS/document_1/document_1.html#_Toc172118878"^^xsd:anyURI ;
    dcat:theme legcons:Item .

C2020A00012:187 a legcons:Item,
        owl:Class,
        dcat:Resource ;
    rdfs:label "Item - I187 136  Export operations must not be carried out while registration suspended"@en-AU ;
    dct:isPartOf C2020A00012:185 ;
    dct:isReferencedBy C2020A00012: ;
    rdfs:comment "136  Export operations must not be carried out while registration suspended - Abrievated Graph Key: I187"@en-AU ;
    skos:definition "136  Export operations must not be carried out while registration suspended"@en-AU ;
    skos:narrower C2020A00012:185 ;
    skos:prefLabel "Item I187"@en-AU ;
    dcat:accessURL <https://www.legislation.gov.au/C2020A00012/2024-07-10/2024-07-10/text/original/epub/OEBPS/document_1/document_1.html#_Toc172118879> ;
    dcat:landingPage "https://www.legislation.gov.au/C2020A00012/2024-07-10/2024-07-10/text/original/epub/OEBPS/document_1/document_1.html#_Toc172118879"^^xsd:anyURI ;
    dcat:theme legcons:Item .

C2020A00012:19 a legcons:Item,
        owl:Class,
        dcat:Resource ;
    rdfs:label "Item - I19 15  Meaning of entered for export"@en-AU ;
    dct:isPartOf C2020A00012:1 ;
    dct:isReferencedBy C2020A00012: ;
    rdfs:comment "15  Meaning of entered for export - Abrievated Graph Key: I19"@en-AU ;
    skos:definition "15  Meaning of entered for export"@en-AU ;
    skos:narrower C2020A00012:1 ;
    skos:prefLabel "Item I19"@en-AU ;
    dcat:accessURL <https://www.legislation.gov.au/C2020A00012/2024-07-10/2024-07-10/text/original/epub/OEBPS/document_1/document_1.html#_Toc172118711> ;
    dcat:landingPage "https://www.legislation.gov.au/C2020A00012/2024-07-10/2024-07-10/text/original/epub/OEBPS/document_1/document_1.html#_Toc172118711"^^xsd:anyURI ;
    dcat:theme legcons:Item .

C2020A00012:190 a legcons:Item,
        owl:Class,
        dcat:Resource ;
    rdfs:label "Item - I190 137  Occupier may request revocation"@en-AU ;
    dct:isPartOf C2020A00012:189 ;
    dct:isReferencedBy C2020A00012: ;
    rdfs:comment "137  Occupier may request revocation - Abrievated Graph Key: I190"@en-AU ;
    skos:definition "137  Occupier may request revocation"@en-AU ;
    skos:narrower C2020A00012:189 ;
    skos:prefLabel "Item I190"@en-AU ;
    dcat:accessURL <https://www.legislation.gov.au/C2020A00012/2024-07-10/2024-07-10/text/original/epub/OEBPS/document_1/document_1.html#_Toc172118882> ;
    dcat:landingPage "https://www.legislation.gov.au/C2020A00012/2024-07-10/2024-07-10/text/original/epub/OEBPS/document_1/document_1.html#_Toc172118882"^^xsd:anyURI ;
    dcat:theme legcons:Item .

C2020A00012:192 a legcons:Item,
        owl:Class,
        dcat:Resource ;
    rdfs:label "Item - I192 138  Grounds for revocationgeneral"@en-AU ;
    dct:isPartOf C2020A00012:191 ;
    dct:isReferencedBy C2020A00012: ;
    rdfs:comment "138  Grounds for revocationgeneral - Abrievated Graph Key: I192"@en-AU ;
    skos:definition "138  Grounds for revocationgeneral"@en-AU ;
    skos:narrower C2020A00012:191 ;
    skos:prefLabel "Item I192"@en-AU ;
    dcat:accessURL <https://www.legislation.gov.au/C2020A00012/2024-07-10/2024-07-10/text/original/epub/OEBPS/document_1/document_1.html#_Toc172118884> ;
    dcat:landingPage "https://www.legislation.gov.au/C2020A00012/2024-07-10/2024-07-10/text/original/epub/OEBPS/document_1/document_1.html#_Toc172118884"^^xsd:anyURI ;
    dcat:theme legcons:Item .

C2020A00012:193 a legcons:Item,
        owl:Class,
        dcat:Resource ;
    rdfs:label "Item - I193 139  Grounds for revocationoverdue relevant Commonwealth liability"@en-AU ;
    dct:isPartOf C2020A00012:191 ;
    dct:isReferencedBy C2020A00012: ;
    rdfs:comment "139  Grounds for revocationoverdue relevant Commonwealth liability - Abrievated Graph Key: I193"@en-AU ;
    skos:definition "139  Grounds for revocationoverdue relevant Commonwealth liability"@en-AU ;
    skos:narrower C2020A00012:191 ;
    skos:prefLabel "Item I193"@en-AU ;
    dcat:accessURL <https://www.legislation.gov.au/C2020A00012/2024-07-10/2024-07-10/text/original/epub/OEBPS/document_1/document_1.html#_Toc172118885> ;
    dcat:landingPage "https://www.legislation.gov.au/C2020A00012/2024-07-10/2024-07-10/text/original/epub/OEBPS/document_1/document_1.html#_Toc172118885"^^xsd:anyURI ;
    dcat:theme legcons:Item .

C2020A00012:194 a legcons:Item,
        owl:Class,
        dcat:Resource ;
    rdfs:label "Item - I194 140  Notice of revocation"@en-AU ;
    dct:isPartOf C2020A00012:191 ;
    dct:isReferencedBy C2020A00012: ;
    rdfs:comment "140  Notice of revocation - Abrievated Graph Key: I194"@en-AU ;
    skos:definition "140  Notice of revocation"@en-AU ;
    skos:narrower C2020A00012:191 ;
    skos:prefLabel "Item I194"@en-AU ;
    dcat:accessURL <https://www.legislation.gov.au/C2020A00012/2024-07-10/2024-07-10/text/original/epub/OEBPS/document_1/document_1.html#_Toc172118886> ;
    dcat:landingPage "https://www.legislation.gov.au/C2020A00012/2024-07-10/2024-07-10/text/original/epub/OEBPS/document_1/document_1.html#_Toc172118886"^^xsd:anyURI ;
    dcat:theme legcons:Item .

C2020A00012:196 a legcons:Item,
        owl:Class,
        dcat:Resource ;
    rdfs:label "Item - I196 141  Export operations must not be carried out after registration of establishment revoked"@en-AU ;
    dct:isPartOf C2020A00012:195 ;
    dct:isReferencedBy C2020A00012: ;
    rdfs:comment "141  Export operations must not be carried out after registration of establishment revoked - Abrievated Graph Key: I196"@en-AU ;
    skos:definition "141  Export operations must not be carried out after registration of establishment revoked"@en-AU ;
    skos:narrower C2020A00012:195 ;
    skos:prefLabel "Item I196"@en-AU ;
    dcat:accessURL <https://www.legislation.gov.au/C2020A00012/2024-07-10/2024-07-10/text/original/epub/OEBPS/document_1/document_1.html#_Toc172118888> ;
    dcat:landingPage "https://www.legislation.gov.au/C2020A00012/2024-07-10/2024-07-10/text/original/epub/OEBPS/document_1/document_1.html#_Toc172118888"^^xsd:anyURI ;
    dcat:theme legcons:Item .

C2020A00012:197 a legcons:Item,
        owl:Class,
        dcat:Resource ;
    rdfs:label "Item - I197 142  Secretary may require action to be taken after registration revoked"@en-AU ;
    dct:isPartOf C2020A00012:195 ;
    dct:isReferencedBy C2020A00012: ;
    rdfs:comment "142  Secretary may require action to be taken after registration revoked - Abrievated Graph Key: I197"@en-AU ;
    skos:definition "142  Secretary may require action to be taken after registration revoked"@en-AU ;
    skos:narrower C2020A00012:195 ;
    skos:prefLabel "Item I197"@en-AU ;
    dcat:accessURL <https://www.legislation.gov.au/C2020A00012/2024-07-10/2024-07-10/text/original/epub/OEBPS/document_1/document_1.html#_Toc172118889> ;
    dcat:landingPage "https://www.legislation.gov.au/C2020A00012/2024-07-10/2024-07-10/text/original/epub/OEBPS/document_1/document_1.html#_Toc172118889"^^xsd:anyURI ;
    dcat:theme legcons:Item .

C2020A00012:199 a legcons:Item,
        owl:Class,
        dcat:Resource ;
    rdfs:label "Item - I199 143  Export operations not covered by registration must not be carried out"@en-AU ;
    dct:isPartOf C2020A00012:198 ;
    dct:isReferencedBy C2020A00012: ;
    rdfs:comment "143  Export operations not covered by registration must not be carried out - Abrievated Graph Key: I199"@en-AU ;
    skos:definition "143  Export operations not covered by registration must not be carried out"@en-AU ;
    skos:narrower C2020A00012:198 ;
    skos:prefLabel "Item I199"@en-AU ;
    dcat:accessURL <https://www.legislation.gov.au/C2020A00012/2024-07-10/2024-07-10/text/original/epub/OEBPS/document_1/document_1.html#_Toc172118891> ;
    dcat:landingPage "https://www.legislation.gov.au/C2020A00012/2024-07-10/2024-07-10/text/original/epub/OEBPS/document_1/document_1.html#_Toc172118891"^^xsd:anyURI ;
    dcat:theme legcons:Item .

C2020A00012:2 a legcons:Part,
        owl:Class,
        dcat:Resource ;
    rdfs:label "Part - P2 Part 1 Preliminary"@en-AU ;
    dct:isPartOf C2020A00012:1 ;
    dct:isReferencedBy C2020A00012: ;
    rdfs:comment "Part 1 Preliminary - Abrievated Graph Key: P2"@en-AU ;
    skos:definition "Part 1 Preliminary"@en-AU ;
    skos:narrower C2020A00012:1 ;
    skos:prefLabel "Part P2"@en-AU ;
    dcat:accessURL <https://www.legislation.gov.au/C2020A00012/2024-07-10/2024-07-10/text/original/epub/OEBPS/document_1/document_1.html#_Toc172118694> ;
    dcat:landingPage "https://www.legislation.gov.au/C2020A00012/2024-07-10/2024-07-10/text/original/epub/OEBPS/document_1/document_1.html#_Toc172118694"^^xsd:anyURI ;
    dcat:theme legcons:Part .

C2020A00012:20 a legcons:Item,
        owl:Class,
        dcat:Resource ;
    rdfs:label "Item - I20 16  Meaning of export operations"@en-AU ;
    dct:isPartOf C2020A00012:1 ;
    dct:isReferencedBy C2020A00012: ;
    rdfs:comment "16  Meaning of export operations - Abrievated Graph Key: I20"@en-AU ;
    skos:definition "16  Meaning of export operations"@en-AU ;
    skos:narrower C2020A00012:1 ;
    skos:prefLabel "Item I20"@en-AU ;
    dcat:accessURL <https://www.legislation.gov.au/C2020A00012/2024-07-10/2024-07-10/text/original/epub/OEBPS/document_1/document_1.html#_Toc172118712> ;
    dcat:landingPage "https://www.legislation.gov.au/C2020A00012/2024-07-10/2024-07-10/text/original/epub/OEBPS/document_1/document_1.html#_Toc172118712"^^xsd:anyURI ;
    dcat:theme legcons:Item .

C2020A00012:200 a legcons:Item,
        owl:Class,
        dcat:Resource ;
    rdfs:label "Item - I200 144  Conditions of registration must not be contravened"@en-AU ;
    dct:isPartOf C2020A00012:198 ;
    dct:isReferencedBy C2020A00012: ;
    rdfs:comment "144  Conditions of registration must not be contravened - Abrievated Graph Key: I200"@en-AU ;
    skos:definition "144  Conditions of registration must not be contravened"@en-AU ;
    skos:narrower C2020A00012:198 ;
    skos:prefLabel "Item I200"@en-AU ;
    dcat:accessURL <https://www.legislation.gov.au/C2020A00012/2024-07-10/2024-07-10/text/original/epub/OEBPS/document_1/document_1.html#_Toc172118892> ;
    dcat:landingPage "https://www.legislation.gov.au/C2020A00012/2024-07-10/2024-07-10/text/original/epub/OEBPS/document_1/document_1.html#_Toc172118892"^^xsd:anyURI ;
    dcat:theme legcons:Item .

C2020A00012:201 a legcons:Item,
        owl:Class,
        dcat:Resource ;
    rdfs:label "Item - I201 145  Additional or corrected information in relation to application for registration etc"@en-AU ;
    dct:isPartOf C2020A00012:198 ;
    dct:isReferencedBy C2020A00012: ;
    rdfs:comment "145  Additional or corrected information in relation to application for registration etc - Abrievated Graph Key: I201"@en-AU ;
    skos:definition "145  Additional or corrected information in relation to application for registration etc"@en-AU ;
    skos:narrower C2020A00012:198 ;
    skos:prefLabel "Item I201"@en-AU ;
    dcat:accessURL <https://www.legislation.gov.au/C2020A00012/2024-07-10/2024-07-10/text/original/epub/OEBPS/document_1/document_1.html#_Toc172118893> ;
    dcat:landingPage "https://www.legislation.gov.au/C2020A00012/2024-07-10/2024-07-10/text/original/epub/OEBPS/document_1/document_1.html#_Toc172118893"^^xsd:anyURI ;
    dcat:theme legcons:Item .

C2020A00012:202 a legcons:Item,
        owl:Class,
        dcat:Resource ;
    rdfs:label "Item - I202 146  Notice of changes to occupier of registered establishment"@en-AU ;
    dct:isPartOf C2020A00012:198 ;
    dct:isReferencedBy C2020A00012: ;
    rdfs:comment "146  Notice of changes to occupier of registered establishment - Abrievated Graph Key: I202"@en-AU ;
    skos:definition "146  Notice of changes to occupier of registered establishment"@en-AU ;
    skos:narrower C2020A00012:198 ;
    skos:prefLabel "Item I202"@en-AU ;
    dcat:accessURL <https://www.legislation.gov.au/C2020A00012/2024-07-10/2024-07-10/text/original/epub/OEBPS/document_1/document_1.html#_Toc172118894> ;
    dcat:landingPage "https://www.legislation.gov.au/C2020A00012/2024-07-10/2024-07-10/text/original/epub/OEBPS/document_1/document_1.html#_Toc172118894"^^xsd:anyURI ;
    dcat:theme legcons:Item .

C2020A00012:203 a legcons:Item,
        owl:Class,
        dcat:Resource ;
    rdfs:label "Item - I203 147  Notice of person ceasing to be occupier of registered establishment"@en-AU ;
    dct:isPartOf C2020A00012:198 ;
    dct:isReferencedBy C2020A00012: ;
    rdfs:comment "147  Notice of person ceasing to be occupier of registered establishment - Abrievated Graph Key: I203"@en-AU ;
    skos:definition "147  Notice of person ceasing to be occupier of registered establishment"@en-AU ;
    skos:narrower C2020A00012:198 ;
    skos:prefLabel "Item I203"@en-AU ;
    dcat:accessURL <https://www.legislation.gov.au/C2020A00012/2024-07-10/2024-07-10/text/original/epub/OEBPS/document_1/document_1.html#_Toc172118895> ;
    dcat:landingPage "https://www.legislation.gov.au/C2020A00012/2024-07-10/2024-07-10/text/original/epub/OEBPS/document_1/document_1.html#_Toc172118895"^^xsd:anyURI ;
    dcat:theme legcons:Item .

C2020A00012:205 a legcons:Item,
        owl:Class,
        dcat:Resource ;
    rdfs:label "Item - I205 148  Register of registered establishments"@en-AU ;
    dct:isPartOf C2020A00012:204 ;
    dct:isReferencedBy C2020A00012: ;
    rdfs:comment "148  Register of registered establishments - Abrievated Graph Key: I205"@en-AU ;
    skos:definition "148  Register of registered establishments"@en-AU ;
    skos:narrower C2020A00012:204 ;
    skos:prefLabel "Item I205"@en-AU ;
    dcat:accessURL <https://www.legislation.gov.au/C2020A00012/2024-07-10/2024-07-10/text/original/epub/OEBPS/document_1/document_1.html#_Toc172118897> ;
    dcat:landingPage "https://www.legislation.gov.au/C2020A00012/2024-07-10/2024-07-10/text/original/epub/OEBPS/document_1/document_1.html#_Toc172118897"^^xsd:anyURI ;
    dcat:theme legcons:Item .

C2020A00012:208 a legcons:Item,
        owl:Class,
        dcat:Resource ;
    rdfs:label "Item - I208 149  Simplified outline of this Chapter"@en-AU ;
    dct:isPartOf C2020A00012:207 ;
    dct:isReferencedBy C2020A00012: ;
    rdfs:comment "149  Simplified outline of this Chapter - Abrievated Graph Key: I208"@en-AU ;
    skos:definition "149  Simplified outline of this Chapter"@en-AU ;
    skos:narrower C2020A00012:207 ;
    skos:prefLabel "Item I208"@en-AU ;
    dcat:accessURL <https://www.legislation.gov.au/C2020A00012/2024-07-10/2024-07-10/text/original/epub/OEBPS/document_1/document_1.html#_Toc172118900> ;
    dcat:landingPage "https://www.legislation.gov.au/C2020A00012/2024-07-10/2024-07-10/text/original/epub/OEBPS/document_1/document_1.html#_Toc172118900"^^xsd:anyURI ;
    dcat:theme legcons:Item .

C2020A00012:21 a legcons:Item,
        owl:Class,
        dcat:Resource ;
    rdfs:label "Item - I21 17  Meaning of installation"@en-AU ;
    dct:isPartOf C2020A00012:1 ;
    dct:isReferencedBy C2020A00012: ;
    rdfs:comment "17  Meaning of installation - Abrievated Graph Key: I21"@en-AU ;
    skos:definition "17  Meaning of installation"@en-AU ;
    skos:narrower C2020A00012:1 ;
    skos:prefLabel "Item I21"@en-AU ;
    dcat:accessURL <https://www.legislation.gov.au/C2020A00012/2024-07-10/2024-07-10/text/original/epub/OEBPS/document_1/document_1.html#_Toc172118713> ;
    dcat:landingPage "https://www.legislation.gov.au/C2020A00012/2024-07-10/2024-07-10/text/original/epub/OEBPS/document_1/document_1.html#_Toc172118713"^^xsd:anyURI ;
    dcat:theme legcons:Item .

C2020A00012:210 a legcons:Item,
        owl:Class,
        dcat:Resource ;
    rdfs:label "Item - I210 150  Application for approval of proposed arrangement"@en-AU ;
    dct:isPartOf C2020A00012:209 ;
    dct:isReferencedBy C2020A00012: ;
    rdfs:comment "150  Application for approval of proposed arrangement - Abrievated Graph Key: I210"@en-AU ;
    skos:definition "150  Application for approval of proposed arrangement"@en-AU ;
    skos:narrower C2020A00012:209 ;
    skos:prefLabel "Item I210"@en-AU ;
    dcat:accessURL <https://www.legislation.gov.au/C2020A00012/2024-07-10/2024-07-10/text/original/epub/OEBPS/document_1/document_1.html#_Toc172118902> ;
    dcat:landingPage "https://www.legislation.gov.au/C2020A00012/2024-07-10/2024-07-10/text/original/epub/OEBPS/document_1/document_1.html#_Toc172118902"^^xsd:anyURI ;
    dcat:theme legcons:Item .

C2020A00012:211 a legcons:Item,
        owl:Class,
        dcat:Resource ;
    rdfs:label "Item - I211 151  Secretary must decide whether to approve proposed arrangement"@en-AU ;
    dct:isPartOf C2020A00012:209 ;
    dct:isReferencedBy C2020A00012: ;
    rdfs:comment "151  Secretary must decide whether to approve proposed arrangement - Abrievated Graph Key: I211"@en-AU ;
    skos:definition "151  Secretary must decide whether to approve proposed arrangement"@en-AU ;
    skos:narrower C2020A00012:209 ;
    skos:prefLabel "Item I211"@en-AU ;
    dcat:accessURL <https://www.legislation.gov.au/C2020A00012/2024-07-10/2024-07-10/text/original/epub/OEBPS/document_1/document_1.html#_Toc172118903> ;
    dcat:landingPage "https://www.legislation.gov.au/C2020A00012/2024-07-10/2024-07-10/text/original/epub/OEBPS/document_1/document_1.html#_Toc172118903"^^xsd:anyURI ;
    dcat:theme legcons:Item .

C2020A00012:212 a legcons:Item,
        owl:Class,
        dcat:Resource ;
    rdfs:label "Item - I212 152  Conditions of approved arrangement"@en-AU ;
    dct:isPartOf C2020A00012:209 ;
    dct:isReferencedBy C2020A00012: ;
    rdfs:comment "152  Conditions of approved arrangement - Abrievated Graph Key: I212"@en-AU ;
    skos:definition "152  Conditions of approved arrangement"@en-AU ;
    skos:narrower C2020A00012:209 ;
    skos:prefLabel "Item I212"@en-AU ;
    dcat:accessURL <https://www.legislation.gov.au/C2020A00012/2024-07-10/2024-07-10/text/original/epub/OEBPS/document_1/document_1.html#_Toc172118904> ;
    dcat:landingPage "https://www.legislation.gov.au/C2020A00012/2024-07-10/2024-07-10/text/original/epub/OEBPS/document_1/document_1.html#_Toc172118904"^^xsd:anyURI ;
    dcat:theme legcons:Item .

C2020A00012:213 a legcons:Item,
        owl:Class,
        dcat:Resource ;
    rdfs:label "Item - I213 153  Notice of decision"@en-AU ;
    dct:isPartOf C2020A00012:209 ;
    dct:isReferencedBy C2020A00012: ;
    rdfs:comment "153  Notice of decision - Abrievated Graph Key: I213"@en-AU ;
    skos:definition "153  Notice of decision"@en-AU ;
    skos:narrower C2020A00012:209 ;
    skos:prefLabel "Item I213"@en-AU ;
    dcat:accessURL <https://www.legislation.gov.au/C2020A00012/2024-07-10/2024-07-10/text/original/epub/OEBPS/document_1/document_1.html#_Toc172118905> ;
    dcat:landingPage "https://www.legislation.gov.au/C2020A00012/2024-07-10/2024-07-10/text/original/epub/OEBPS/document_1/document_1.html#_Toc172118905"^^xsd:anyURI ;
    dcat:theme legcons:Item .

C2020A00012:214 a legcons:Item,
        owl:Class,
        dcat:Resource ;
    rdfs:label "Item - I214 154  Period of effect of approved arrangement"@en-AU ;
    dct:isPartOf C2020A00012:209 ;
    dct:isReferencedBy C2020A00012: ;
    rdfs:comment "154  Period of effect of approved arrangement - Abrievated Graph Key: I214"@en-AU ;
    skos:definition "154  Period of effect of approved arrangement"@en-AU ;
    skos:narrower C2020A00012:209 ;
    skos:prefLabel "Item I214"@en-AU ;
    dcat:accessURL <https://www.legislation.gov.au/C2020A00012/2024-07-10/2024-07-10/text/original/epub/OEBPS/document_1/document_1.html#_Toc172118906> ;
    dcat:landingPage "https://www.legislation.gov.au/C2020A00012/2024-07-10/2024-07-10/text/original/epub/OEBPS/document_1/document_1.html#_Toc172118906"^^xsd:anyURI ;
    dcat:theme legcons:Item .

C2020A00012:216 a legcons:Item,
        owl:Class,
        dcat:Resource ;
    rdfs:label "Item - I216 155  Application to renew approved arrangement"@en-AU ;
    dct:isPartOf C2020A00012:215 ;
    dct:isReferencedBy C2020A00012: ;
    rdfs:comment "155  Application to renew approved arrangement - Abrievated Graph Key: I216"@en-AU ;
    skos:definition "155  Application to renew approved arrangement"@en-AU ;
    skos:narrower C2020A00012:215 ;
    skos:prefLabel "Item I216"@en-AU ;
    dcat:accessURL <https://www.legislation.gov.au/C2020A00012/2024-07-10/2024-07-10/text/original/epub/OEBPS/document_1/document_1.html#_Toc172118908> ;
    dcat:landingPage "https://www.legislation.gov.au/C2020A00012/2024-07-10/2024-07-10/text/original/epub/OEBPS/document_1/document_1.html#_Toc172118908"^^xsd:anyURI ;
    dcat:theme legcons:Item .

C2020A00012:217 a legcons:Item,
        owl:Class,
        dcat:Resource ;
    rdfs:label "Item - I217 156  Secretary must decide whether to renew approved arrangement"@en-AU ;
    dct:isPartOf C2020A00012:215 ;
    dct:isReferencedBy C2020A00012: ;
    rdfs:comment "156  Secretary must decide whether to renew approved arrangement - Abrievated Graph Key: I217"@en-AU ;
    skos:definition "156  Secretary must decide whether to renew approved arrangement"@en-AU ;
    skos:narrower C2020A00012:215 ;
    skos:prefLabel "Item I217"@en-AU ;
    dcat:accessURL <https://www.legislation.gov.au/C2020A00012/2024-07-10/2024-07-10/text/original/epub/OEBPS/document_1/document_1.html#_Toc172118909> ;
    dcat:landingPage "https://www.legislation.gov.au/C2020A00012/2024-07-10/2024-07-10/text/original/epub/OEBPS/document_1/document_1.html#_Toc172118909"^^xsd:anyURI ;
    dcat:theme legcons:Item .

C2020A00012:218 a legcons:Item,
        owl:Class,
        dcat:Resource ;
    rdfs:label "Item - I218 157  Conditions of renewed approved arrangement"@en-AU ;
    dct:isPartOf C2020A00012:215 ;
    dct:isReferencedBy C2020A00012: ;
    rdfs:comment "157  Conditions of renewed approved arrangement - Abrievated Graph Key: I218"@en-AU ;
    skos:definition "157  Conditions of renewed approved arrangement"@en-AU ;
    skos:narrower C2020A00012:215 ;
    skos:prefLabel "Item I218"@en-AU ;
    dcat:accessURL <https://www.legislation.gov.au/C2020A00012/2024-07-10/2024-07-10/text/original/epub/OEBPS/document_1/document_1.html#_Toc172118910> ;
    dcat:landingPage "https://www.legislation.gov.au/C2020A00012/2024-07-10/2024-07-10/text/original/epub/OEBPS/document_1/document_1.html#_Toc172118910"^^xsd:anyURI ;
    dcat:theme legcons:Item .

C2020A00012:219 a legcons:Item,
        owl:Class,
        dcat:Resource ;
    rdfs:label "Item - I219 158  Notice of decision"@en-AU ;
    dct:isPartOf C2020A00012:215 ;
    dct:isReferencedBy C2020A00012: ;
    rdfs:comment "158  Notice of decision - Abrievated Graph Key: I219"@en-AU ;
    skos:definition "158  Notice of decision"@en-AU ;
    skos:narrower C2020A00012:215 ;
    skos:prefLabel "Item I219"@en-AU ;
    dcat:accessURL <https://www.legislation.gov.au/C2020A00012/2024-07-10/2024-07-10/text/original/epub/OEBPS/document_1/document_1.html#_Toc172118911> ;
    dcat:landingPage "https://www.legislation.gov.au/C2020A00012/2024-07-10/2024-07-10/text/original/epub/OEBPS/document_1/document_1.html#_Toc172118911"^^xsd:anyURI ;
    dcat:theme legcons:Item .

C2020A00012:22 a legcons:Item,
        owl:Class,
        dcat:Resource ;
    rdfs:label "Item - I22 18  Meaning of integrity"@en-AU ;
    dct:isPartOf C2020A00012:1 ;
    dct:isReferencedBy C2020A00012: ;
    rdfs:comment "18  Meaning of integrity - Abrievated Graph Key: I22"@en-AU ;
    skos:definition "18  Meaning of integrity"@en-AU ;
    skos:narrower C2020A00012:1 ;
    skos:prefLabel "Item I22"@en-AU ;
    dcat:accessURL <https://www.legislation.gov.au/C2020A00012/2024-07-10/2024-07-10/text/original/epub/OEBPS/document_1/document_1.html#_Toc172118714> ;
    dcat:landingPage "https://www.legislation.gov.au/C2020A00012/2024-07-10/2024-07-10/text/original/epub/OEBPS/document_1/document_1.html#_Toc172118714"^^xsd:anyURI ;
    dcat:theme legcons:Item .

C2020A00012:223 a legcons:Item,
        owl:Class,
        dcat:Resource ;
    rdfs:label "Item - I223 159  Holder may make non significant variations of approved arrangement"@en-AU ;
    dct:isPartOf C2020A00012:222 ;
    dct:isReferencedBy C2020A00012: ;
    rdfs:comment "159  Holder may make non significant variations of approved arrangement - Abrievated Graph Key: I223"@en-AU ;
    skos:definition "159  Holder may make non significant variations of approved arrangement"@en-AU ;
    skos:narrower C2020A00012:222 ;
    skos:prefLabel "Item I223"@en-AU ;
    dcat:accessURL <https://www.legislation.gov.au/C2020A00012/2024-07-10/2024-07-10/text/original/epub/OEBPS/document_1/document_1.html#_Toc172118915> ;
    dcat:landingPage "https://www.legislation.gov.au/C2020A00012/2024-07-10/2024-07-10/text/original/epub/OEBPS/document_1/document_1.html#_Toc172118915"^^xsd:anyURI ;
    dcat:theme legcons:Item .

C2020A00012:224 a legcons:Item,
        owl:Class,
        dcat:Resource ;
    rdfs:label "Item - I224 160  Date of effect of varied approved arrangement"@en-AU ;
    dct:isPartOf C2020A00012:222 ;
    dct:isReferencedBy C2020A00012: ;
    rdfs:comment "160  Date of effect of varied approved arrangement - Abrievated Graph Key: I224"@en-AU ;
    skos:definition "160  Date of effect of varied approved arrangement"@en-AU ;
    skos:narrower C2020A00012:222 ;
    skos:prefLabel "Item I224"@en-AU ;
    dcat:accessURL <https://www.legislation.gov.au/C2020A00012/2024-07-10/2024-07-10/text/original/epub/OEBPS/document_1/document_1.html#_Toc172118916> ;
    dcat:landingPage "https://www.legislation.gov.au/C2020A00012/2024-07-10/2024-07-10/text/original/epub/OEBPS/document_1/document_1.html#_Toc172118916"^^xsd:anyURI ;
    dcat:theme legcons:Item .

C2020A00012:226 a legcons:Item,
        owl:Class,
        dcat:Resource ;
    rdfs:label "Item - I226 161  Application by holder for approval of approved alternative regulatory arrangement or other significant variation or to vary conditions"@en-AU ;
    dct:isPartOf C2020A00012:225 ;
    dct:isReferencedBy C2020A00012: ;
    rdfs:comment "161  Application by holder for approval of approved alternative regulatory arrangement or other significant variation or to vary conditions - Abrievated Graph Key: I226"@en-AU ;
    skos:definition "161  Application by holder for approval of approved alternative regulatory arrangement or other significant variation or to vary conditions"@en-AU ;
    skos:narrower C2020A00012:225 ;
    skos:prefLabel "Item I226"@en-AU ;
    dcat:accessURL <https://www.legislation.gov.au/C2020A00012/2024-07-10/2024-07-10/text/original/epub/OEBPS/document_1/document_1.html#_Toc172118918> ;
    dcat:landingPage "https://www.legislation.gov.au/C2020A00012/2024-07-10/2024-07-10/text/original/epub/OEBPS/document_1/document_1.html#_Toc172118918"^^xsd:anyURI ;
    dcat:theme legcons:Item .

C2020A00012:227 a legcons:Item,
        owl:Class,
        dcat:Resource ;
    rdfs:label "Item - I227 162  Notice of variation"@en-AU ;
    dct:isPartOf C2020A00012:225 ;
    dct:isReferencedBy C2020A00012: ;
    rdfs:comment "162  Notice of variation - Abrievated Graph Key: I227"@en-AU ;
    skos:definition "162  Notice of variation"@en-AU ;
    skos:narrower C2020A00012:225 ;
    skos:prefLabel "Item I227"@en-AU ;
    dcat:accessURL <https://www.legislation.gov.au/C2020A00012/2024-07-10/2024-07-10/text/original/epub/OEBPS/document_1/document_1.html#_Toc172118919> ;
    dcat:landingPage "https://www.legislation.gov.au/C2020A00012/2024-07-10/2024-07-10/text/original/epub/OEBPS/document_1/document_1.html#_Toc172118919"^^xsd:anyURI ;
    dcat:theme legcons:Item .

C2020A00012:228 a legcons:Item,
        owl:Class,
        dcat:Resource ;
    rdfs:label "Item - I228 163  Varied approved arrangement must not be implemented unless variation approved etc"@en-AU ;
    dct:isPartOf C2020A00012:225 ;
    dct:isReferencedBy C2020A00012: ;
    rdfs:comment "163  Varied approved arrangement must not be implemented unless variation approved etc - Abrievated Graph Key: I228"@en-AU ;
    skos:definition "163  Varied approved arrangement must not be implemented unless variation approved etc"@en-AU ;
    skos:narrower C2020A00012:225 ;
    skos:prefLabel "Item I228"@en-AU ;
    dcat:accessURL <https://www.legislation.gov.au/C2020A00012/2024-07-10/2024-07-10/text/original/epub/OEBPS/document_1/document_1.html#_Toc172118920> ;
    dcat:landingPage "https://www.legislation.gov.au/C2020A00012/2024-07-10/2024-07-10/text/original/epub/OEBPS/document_1/document_1.html#_Toc172118920"^^xsd:anyURI ;
    dcat:theme legcons:Item .

C2020A00012:23 a legcons:Item,
        owl:Class,
        dcat:Resource ;
    rdfs:label "Item - I23 19  Meaning of occupier"@en-AU ;
    dct:isPartOf C2020A00012:1 ;
    dct:isReferencedBy C2020A00012: ;
    rdfs:comment "19  Meaning of occupier - Abrievated Graph Key: I23"@en-AU ;
    skos:definition "19  Meaning of occupier"@en-AU ;
    skos:narrower C2020A00012:1 ;
    skos:prefLabel "Item I23"@en-AU ;
    dcat:accessURL <https://www.legislation.gov.au/C2020A00012/2024-07-10/2024-07-10/text/original/epub/OEBPS/document_1/document_1.html#_Toc172118715> ;
    dcat:landingPage "https://www.legislation.gov.au/C2020A00012/2024-07-10/2024-07-10/text/original/epub/OEBPS/document_1/document_1.html#_Toc172118715"^^xsd:anyURI ;
    dcat:theme legcons:Item .

C2020A00012:230 a legcons:Item,
        owl:Class,
        dcat:Resource ;
    rdfs:label "Item - I230 164  Matters to which regard must be had in considering whether proposed variation of approved arrangement is significant"@en-AU ;
    dct:isPartOf C2020A00012:229 ;
    dct:isReferencedBy C2020A00012: ;
    rdfs:comment "164  Matters to which regard must be had in considering whether proposed variation of approved arrangement is significant - Abrievated Graph Key: I230"@en-AU ;
    skos:definition "164  Matters to which regard must be had in considering whether proposed variation of approved arrangement is significant"@en-AU ;
    skos:narrower C2020A00012:229 ;
    skos:prefLabel "Item I230"@en-AU ;
    dcat:accessURL <https://www.legislation.gov.au/C2020A00012/2024-07-10/2024-07-10/text/original/epub/OEBPS/document_1/document_1.html#_Toc172118922> ;
    dcat:landingPage "https://www.legislation.gov.au/C2020A00012/2024-07-10/2024-07-10/text/original/epub/OEBPS/document_1/document_1.html#_Toc172118922"^^xsd:anyURI ;
    dcat:theme legcons:Item .

C2020A00012:232 a legcons:Item,
        owl:Class,
        dcat:Resource ;
    rdfs:label "Item - I232 165  Secretary may require approved arrangement to be varied or make certain variations of approved arrangement"@en-AU ;
    dct:isPartOf C2020A00012:231 ;
    dct:isReferencedBy C2020A00012: ;
    rdfs:comment "165  Secretary may require approved arrangement to be varied or make certain variations of approved arrangement - Abrievated Graph Key: I232"@en-AU ;
    skos:definition "165  Secretary may require approved arrangement to be varied or make certain variations of approved arrangement"@en-AU ;
    skos:narrower C2020A00012:231 ;
    skos:prefLabel "Item I232"@en-AU ;
    dcat:accessURL <https://www.legislation.gov.au/C2020A00012/2024-07-10/2024-07-10/text/original/epub/OEBPS/document_1/document_1.html#_Toc172118924> ;
    dcat:landingPage "https://www.legislation.gov.au/C2020A00012/2024-07-10/2024-07-10/text/original/epub/OEBPS/document_1/document_1.html#_Toc172118924"^^xsd:anyURI ;
    dcat:theme legcons:Item .

C2020A00012:233 a legcons:Item,
        owl:Class,
        dcat:Resource ;
    rdfs:label "Item - I233 166  Variations required by the Secretary"@en-AU ;
    dct:isPartOf C2020A00012:231 ;
    dct:isReferencedBy C2020A00012: ;
    rdfs:comment "166  Variations required by the Secretary - Abrievated Graph Key: I233"@en-AU ;
    skos:definition "166  Variations required by the Secretary"@en-AU ;
    skos:narrower C2020A00012:231 ;
    skos:prefLabel "Item I233"@en-AU ;
    dcat:accessURL <https://www.legislation.gov.au/C2020A00012/2024-07-10/2024-07-10/text/original/epub/OEBPS/document_1/document_1.html#_Toc172118925> ;
    dcat:landingPage "https://www.legislation.gov.au/C2020A00012/2024-07-10/2024-07-10/text/original/epub/OEBPS/document_1/document_1.html#_Toc172118925"^^xsd:anyURI ;
    dcat:theme legcons:Item .

C2020A00012:234 a legcons:Item,
        owl:Class,
        dcat:Resource ;
    rdfs:label "Item - I234 167  Varied approved arrangement must not be implemented unless approved etc"@en-AU ;
    dct:isPartOf C2020A00012:231 ;
    dct:isReferencedBy C2020A00012: ;
    rdfs:comment "167  Varied approved arrangement must not be implemented unless approved etc - Abrievated Graph Key: I234"@en-AU ;
    skos:definition "167  Varied approved arrangement must not be implemented unless approved etc"@en-AU ;
    skos:narrower C2020A00012:231 ;
    skos:prefLabel "Item I234"@en-AU ;
    dcat:accessURL <https://www.legislation.gov.au/C2020A00012/2024-07-10/2024-07-10/text/original/epub/OEBPS/document_1/document_1.html#_Toc172118926> ;
    dcat:landingPage "https://www.legislation.gov.au/C2020A00012/2024-07-10/2024-07-10/text/original/epub/OEBPS/document_1/document_1.html#_Toc172118926"^^xsd:anyURI ;
    dcat:theme legcons:Item .

C2020A00012:235 a legcons:Item,
        owl:Class,
        dcat:Resource ;
    rdfs:label "Item - I235 168  Notice of variations made by the Secretary"@en-AU ;
    dct:isPartOf C2020A00012:231 ;
    dct:isReferencedBy C2020A00012: ;
    rdfs:comment "168  Notice of variations made by the Secretary - Abrievated Graph Key: I235"@en-AU ;
    skos:definition "168  Notice of variations made by the Secretary"@en-AU ;
    skos:narrower C2020A00012:231 ;
    skos:prefLabel "Item I235"@en-AU ;
    dcat:accessURL <https://www.legislation.gov.au/C2020A00012/2024-07-10/2024-07-10/text/original/epub/OEBPS/document_1/document_1.html#_Toc172118927> ;
    dcat:landingPage "https://www.legislation.gov.au/C2020A00012/2024-07-10/2024-07-10/text/original/epub/OEBPS/document_1/document_1.html#_Toc172118927"^^xsd:anyURI ;
    dcat:theme legcons:Item .

C2020A00012:238 a legcons:Item,
        owl:Class,
        dcat:Resource ;
    rdfs:label "Item - I238 169  Holder may request suspension"@en-AU ;
    dct:isPartOf C2020A00012:237 ;
    dct:isReferencedBy C2020A00012: ;
    rdfs:comment "169  Holder may request suspension - Abrievated Graph Key: I238"@en-AU ;
    skos:definition "169  Holder may request suspension"@en-AU ;
    skos:narrower C2020A00012:237 ;
    skos:prefLabel "Item I238"@en-AU ;
    dcat:accessURL <https://www.legislation.gov.au/C2020A00012/2024-07-10/2024-07-10/text/original/epub/OEBPS/document_1/document_1.html#_Toc172118930> ;
    dcat:landingPage "https://www.legislation.gov.au/C2020A00012/2024-07-10/2024-07-10/text/original/epub/OEBPS/document_1/document_1.html#_Toc172118930"^^xsd:anyURI ;
    dcat:theme legcons:Item .

C2020A00012:239 a legcons:Item,
        owl:Class,
        dcat:Resource ;
    rdfs:label "Item - I239 170  Request to revoke suspension"@en-AU ;
    dct:isPartOf C2020A00012:237 ;
    dct:isReferencedBy C2020A00012: ;
    rdfs:comment "170  Request to revoke suspension - Abrievated Graph Key: I239"@en-AU ;
    skos:definition "170  Request to revoke suspension"@en-AU ;
    skos:narrower C2020A00012:237 ;
    skos:prefLabel "Item I239"@en-AU ;
    dcat:accessURL <https://www.legislation.gov.au/C2020A00012/2024-07-10/2024-07-10/text/original/epub/OEBPS/document_1/document_1.html#_Toc172118931> ;
    dcat:landingPage "https://www.legislation.gov.au/C2020A00012/2024-07-10/2024-07-10/text/original/epub/OEBPS/document_1/document_1.html#_Toc172118931"^^xsd:anyURI ;
    dcat:theme legcons:Item .

C2020A00012:24 a legcons:Division,
        owl:Class,
        dcat:Resource ;
    rdfs:label "Division - D24 Division 2 Other interpretation provisions"@en-AU ;
    dct:isPartOf C2020A00012:1 ;
    dct:isReferencedBy C2020A00012: ;
    rdfs:comment "Division 2 Other interpretation provisions - Abrievated Graph Key: D24"@en-AU ;
    skos:definition "Division 2 Other interpretation provisions"@en-AU ;
    skos:narrower C2020A00012:1 ;
    skos:prefLabel "Division D24"@en-AU ;
    dcat:accessURL <https://www.legislation.gov.au/C2020A00012/2024-07-10/2024-07-10/text/original/epub/OEBPS/document_1/document_1.html#_Toc172118716> ;
    dcat:landingPage "https://www.legislation.gov.au/C2020A00012/2024-07-10/2024-07-10/text/original/epub/OEBPS/document_1/document_1.html#_Toc172118716"^^xsd:anyURI ;
    dcat:theme legcons:Division .

C2020A00012:241 a legcons:Item,
        owl:Class,
        dcat:Resource ;
    rdfs:label "Item - I241 171  Grounds for suspensiongeneral"@en-AU ;
    dct:isPartOf C2020A00012:240 ;
    dct:isReferencedBy C2020A00012: ;
    rdfs:comment "171  Grounds for suspensiongeneral - Abrievated Graph Key: I241"@en-AU ;
    skos:definition "171  Grounds for suspensiongeneral"@en-AU ;
    skos:narrower C2020A00012:240 ;
    skos:prefLabel "Item I241"@en-AU ;
    dcat:accessURL <https://www.legislation.gov.au/C2020A00012/2024-07-10/2024-07-10/text/original/epub/OEBPS/document_1/document_1.html#_Toc172118933> ;
    dcat:landingPage "https://www.legislation.gov.au/C2020A00012/2024-07-10/2024-07-10/text/original/epub/OEBPS/document_1/document_1.html#_Toc172118933"^^xsd:anyURI ;
    dcat:theme legcons:Item .

C2020A00012:242 a legcons:Item,
        owl:Class,
        dcat:Resource ;
    rdfs:label "Item - I242 172  Grounds for suspensionoverdue relevant Commonwealth liability"@en-AU ;
    dct:isPartOf C2020A00012:240 ;
    dct:isReferencedBy C2020A00012: ;
    rdfs:comment "172  Grounds for suspensionoverdue relevant Commonwealth liability - Abrievated Graph Key: I242"@en-AU ;
    skos:definition "172  Grounds for suspensionoverdue relevant Commonwealth liability"@en-AU ;
    skos:narrower C2020A00012:240 ;
    skos:prefLabel "Item I242"@en-AU ;
    dcat:accessURL <https://www.legislation.gov.au/C2020A00012/2024-07-10/2024-07-10/text/original/epub/OEBPS/document_1/document_1.html#_Toc172118934> ;
    dcat:landingPage "https://www.legislation.gov.au/C2020A00012/2024-07-10/2024-07-10/text/original/epub/OEBPS/document_1/document_1.html#_Toc172118934"^^xsd:anyURI ;
    dcat:theme legcons:Item .

C2020A00012:243 a legcons:Item,
        owl:Class,
        dcat:Resource ;
    rdfs:label "Item - I243 173  Notice of suspension"@en-AU ;
    dct:isPartOf C2020A00012:240 ;
    dct:isReferencedBy C2020A00012: ;
    rdfs:comment "173  Notice of suspension - Abrievated Graph Key: I243"@en-AU ;
    skos:definition "173  Notice of suspension"@en-AU ;
    skos:narrower C2020A00012:240 ;
    skos:prefLabel "Item I243"@en-AU ;
    dcat:accessURL <https://www.legislation.gov.au/C2020A00012/2024-07-10/2024-07-10/text/original/epub/OEBPS/document_1/document_1.html#_Toc172118935> ;
    dcat:landingPage "https://www.legislation.gov.au/C2020A00012/2024-07-10/2024-07-10/text/original/epub/OEBPS/document_1/document_1.html#_Toc172118935"^^xsd:anyURI ;
    dcat:theme legcons:Item .

C2020A00012:244 a legcons:Item,
        owl:Class,
        dcat:Resource ;
    rdfs:label "Item - I244 174  Period of suspension"@en-AU ;
    dct:isPartOf C2020A00012:240 ;
    dct:isReferencedBy C2020A00012: ;
    rdfs:comment "174  Period of suspension - Abrievated Graph Key: I244"@en-AU ;
    skos:definition "174  Period of suspension"@en-AU ;
    skos:narrower C2020A00012:240 ;
    skos:prefLabel "Item I244"@en-AU ;
    dcat:accessURL <https://www.legislation.gov.au/C2020A00012/2024-07-10/2024-07-10/text/original/epub/OEBPS/document_1/document_1.html#_Toc172118936> ;
    dcat:landingPage "https://www.legislation.gov.au/C2020A00012/2024-07-10/2024-07-10/text/original/epub/OEBPS/document_1/document_1.html#_Toc172118936"^^xsd:anyURI ;
    dcat:theme legcons:Item .

C2020A00012:245 a legcons:Item,
        owl:Class,
        dcat:Resource ;
    rdfs:label "Item - I245 175  Revocation of suspension"@en-AU ;
    dct:isPartOf C2020A00012:240 ;
    dct:isReferencedBy C2020A00012: ;
    rdfs:comment "175  Revocation of suspension - Abrievated Graph Key: I245"@en-AU ;
    skos:definition "175  Revocation of suspension"@en-AU ;
    skos:narrower C2020A00012:240 ;
    skos:prefLabel "Item I245"@en-AU ;
    dcat:accessURL <https://www.legislation.gov.au/C2020A00012/2024-07-10/2024-07-10/text/original/epub/OEBPS/document_1/document_1.html#_Toc172118937> ;
    dcat:landingPage "https://www.legislation.gov.au/C2020A00012/2024-07-10/2024-07-10/text/original/epub/OEBPS/document_1/document_1.html#_Toc172118937"^^xsd:anyURI ;
    dcat:theme legcons:Item .

C2020A00012:247 a legcons:Item,
        owl:Class,
        dcat:Resource ;
    rdfs:label "Item - I247 176  Effect of suspension"@en-AU ;
    dct:isPartOf C2020A00012:246 ;
    dct:isReferencedBy C2020A00012: ;
    rdfs:comment "176  Effect of suspension - Abrievated Graph Key: I247"@en-AU ;
    skos:definition "176  Effect of suspension"@en-AU ;
    skos:narrower C2020A00012:246 ;
    skos:prefLabel "Item I247"@en-AU ;
    dcat:accessURL <https://www.legislation.gov.au/C2020A00012/2024-07-10/2024-07-10/text/original/epub/OEBPS/document_1/document_1.html#_Toc172118939> ;
    dcat:landingPage "https://www.legislation.gov.au/C2020A00012/2024-07-10/2024-07-10/text/original/epub/OEBPS/document_1/document_1.html#_Toc172118939"^^xsd:anyURI ;
    dcat:theme legcons:Item .

C2020A00012:248 a legcons:Item,
        owl:Class,
        dcat:Resource ;
    rdfs:label "Item - I248 177  Export operations must not be carried out while approved arrangement suspended"@en-AU ;
    dct:isPartOf C2020A00012:246 ;
    dct:isReferencedBy C2020A00012: ;
    rdfs:comment "177  Export operations must not be carried out while approved arrangement suspended - Abrievated Graph Key: I248"@en-AU ;
    skos:definition "177  Export operations must not be carried out while approved arrangement suspended"@en-AU ;
    skos:narrower C2020A00012:246 ;
    skos:prefLabel "Item I248"@en-AU ;
    dcat:accessURL <https://www.legislation.gov.au/C2020A00012/2024-07-10/2024-07-10/text/original/epub/OEBPS/document_1/document_1.html#_Toc172118940> ;
    dcat:landingPage "https://www.legislation.gov.au/C2020A00012/2024-07-10/2024-07-10/text/original/epub/OEBPS/document_1/document_1.html#_Toc172118940"^^xsd:anyURI ;
    dcat:theme legcons:Item .

C2020A00012:25 a legcons:Item,
        owl:Class,
        dcat:Resource ;
    rdfs:label "Item - I25 20  When goods are exported"@en-AU ;
    dct:isPartOf C2020A00012:1 ;
    dct:isReferencedBy C2020A00012: ;
    rdfs:comment "20  When goods are exported - Abrievated Graph Key: I25"@en-AU ;
    skos:definition "20  When goods are exported"@en-AU ;
    skos:narrower C2020A00012:1 ;
    skos:prefLabel "Item I25"@en-AU ;
    dcat:accessURL <https://www.legislation.gov.au/C2020A00012/2024-07-10/2024-07-10/text/original/epub/OEBPS/document_1/document_1.html#_Toc172118717> ;
    dcat:landingPage "https://www.legislation.gov.au/C2020A00012/2024-07-10/2024-07-10/text/original/epub/OEBPS/document_1/document_1.html#_Toc172118717"^^xsd:anyURI ;
    dcat:theme legcons:Item .

C2020A00012:251 a legcons:Item,
        owl:Class,
        dcat:Resource ;
    rdfs:label "Item - I251 178  Holder may request revocation"@en-AU ;
    dct:isPartOf C2020A00012:250 ;
    dct:isReferencedBy C2020A00012: ;
    rdfs:comment "178  Holder may request revocation - Abrievated Graph Key: I251"@en-AU ;
    skos:definition "178  Holder may request revocation"@en-AU ;
    skos:narrower C2020A00012:250 ;
    skos:prefLabel "Item I251"@en-AU ;
    dcat:accessURL <https://www.legislation.gov.au/C2020A00012/2024-07-10/2024-07-10/text/original/epub/OEBPS/document_1/document_1.html#_Toc172118943> ;
    dcat:landingPage "https://www.legislation.gov.au/C2020A00012/2024-07-10/2024-07-10/text/original/epub/OEBPS/document_1/document_1.html#_Toc172118943"^^xsd:anyURI ;
    dcat:theme legcons:Item .

C2020A00012:253 a legcons:Item,
        owl:Class,
        dcat:Resource ;
    rdfs:label "Item - I253 179  Grounds for revocationgeneral"@en-AU ;
    dct:isPartOf C2020A00012:252 ;
    dct:isReferencedBy C2020A00012: ;
    rdfs:comment "179  Grounds for revocationgeneral - Abrievated Graph Key: I253"@en-AU ;
    skos:definition "179  Grounds for revocationgeneral"@en-AU ;
    skos:narrower C2020A00012:252 ;
    skos:prefLabel "Item I253"@en-AU ;
    dcat:accessURL <https://www.legislation.gov.au/C2020A00012/2024-07-10/2024-07-10/text/original/epub/OEBPS/document_1/document_1.html#_Toc172118945> ;
    dcat:landingPage "https://www.legislation.gov.au/C2020A00012/2024-07-10/2024-07-10/text/original/epub/OEBPS/document_1/document_1.html#_Toc172118945"^^xsd:anyURI ;
    dcat:theme legcons:Item .

C2020A00012:254 a legcons:Item,
        owl:Class,
        dcat:Resource ;
    rdfs:label "Item - I254 180  Grounds for revocationoverdue relevant Commonwealth liability"@en-AU ;
    dct:isPartOf C2020A00012:252 ;
    dct:isReferencedBy C2020A00012: ;
    rdfs:comment "180  Grounds for revocationoverdue relevant Commonwealth liability - Abrievated Graph Key: I254"@en-AU ;
    skos:definition "180  Grounds for revocationoverdue relevant Commonwealth liability"@en-AU ;
    skos:narrower C2020A00012:252 ;
    skos:prefLabel "Item I254"@en-AU ;
    dcat:accessURL <https://www.legislation.gov.au/C2020A00012/2024-07-10/2024-07-10/text/original/epub/OEBPS/document_1/document_1.html#_Toc172118946> ;
    dcat:landingPage "https://www.legislation.gov.au/C2020A00012/2024-07-10/2024-07-10/text/original/epub/OEBPS/document_1/document_1.html#_Toc172118946"^^xsd:anyURI ;
    dcat:theme legcons:Item .

C2020A00012:255 a legcons:Item,
        owl:Class,
        dcat:Resource ;
    rdfs:label "Item - I255 181  Notice of revocation"@en-AU ;
    dct:isPartOf C2020A00012:252 ;
    dct:isReferencedBy C2020A00012: ;
    rdfs:comment "181  Notice of revocation - Abrievated Graph Key: I255"@en-AU ;
    skos:definition "181  Notice of revocation"@en-AU ;
    skos:narrower C2020A00012:252 ;
    skos:prefLabel "Item I255"@en-AU ;
    dcat:accessURL <https://www.legislation.gov.au/C2020A00012/2024-07-10/2024-07-10/text/original/epub/OEBPS/document_1/document_1.html#_Toc172118947> ;
    dcat:landingPage "https://www.legislation.gov.au/C2020A00012/2024-07-10/2024-07-10/text/original/epub/OEBPS/document_1/document_1.html#_Toc172118947"^^xsd:anyURI ;
    dcat:theme legcons:Item .

C2020A00012:257 a legcons:Item,
        owl:Class,
        dcat:Resource ;
    rdfs:label "Item - I257 182  Export operations must not be carried out after approved arrangement revoked"@en-AU ;
    dct:isPartOf C2020A00012:256 ;
    dct:isReferencedBy C2020A00012: ;
    rdfs:comment "182  Export operations must not be carried out after approved arrangement revoked - Abrievated Graph Key: I257"@en-AU ;
    skos:definition "182  Export operations must not be carried out after approved arrangement revoked"@en-AU ;
    skos:narrower C2020A00012:256 ;
    skos:prefLabel "Item I257"@en-AU ;
    dcat:accessURL <https://www.legislation.gov.au/C2020A00012/2024-07-10/2024-07-10/text/original/epub/OEBPS/document_1/document_1.html#_Toc172118949> ;
    dcat:landingPage "https://www.legislation.gov.au/C2020A00012/2024-07-10/2024-07-10/text/original/epub/OEBPS/document_1/document_1.html#_Toc172118949"^^xsd:anyURI ;
    dcat:theme legcons:Item .

C2020A00012:258 a legcons:Item,
        owl:Class,
        dcat:Resource ;
    rdfs:label "Item - I258 183  Secretary may require action to be taken after approved arrangement revoked"@en-AU ;
    dct:isPartOf C2020A00012:256 ;
    dct:isReferencedBy C2020A00012: ;
    rdfs:comment "183  Secretary may require action to be taken after approved arrangement revoked - Abrievated Graph Key: I258"@en-AU ;
    skos:definition "183  Secretary may require action to be taken after approved arrangement revoked"@en-AU ;
    skos:narrower C2020A00012:256 ;
    skos:prefLabel "Item I258"@en-AU ;
    dcat:accessURL <https://www.legislation.gov.au/C2020A00012/2024-07-10/2024-07-10/text/original/epub/OEBPS/document_1/document_1.html#_Toc172118950> ;
    dcat:landingPage "https://www.legislation.gov.au/C2020A00012/2024-07-10/2024-07-10/text/original/epub/OEBPS/document_1/document_1.html#_Toc172118950"^^xsd:anyURI ;
    dcat:theme legcons:Item .

C2020A00012:26 a legcons:Item,
        owl:Class,
        dcat:Resource ;
    rdfs:label "Item - I26 21  Persons who manage or control export operations"@en-AU ;
    dct:isPartOf C2020A00012:1 ;
    dct:isReferencedBy C2020A00012: ;
    rdfs:comment "21  Persons who manage or control export operations - Abrievated Graph Key: I26"@en-AU ;
    skos:definition "21  Persons who manage or control export operations"@en-AU ;
    skos:narrower C2020A00012:1 ;
    skos:prefLabel "Item I26"@en-AU ;
    dcat:accessURL <https://www.legislation.gov.au/C2020A00012/2024-07-10/2024-07-10/text/original/epub/OEBPS/document_1/document_1.html#_Toc172118718> ;
    dcat:landingPage "https://www.legislation.gov.au/C2020A00012/2024-07-10/2024-07-10/text/original/epub/OEBPS/document_1/document_1.html#_Toc172118718"^^xsd:anyURI ;
    dcat:theme legcons:Item .

C2020A00012:260 a legcons:Item,
        owl:Class,
        dcat:Resource ;
    rdfs:label "Item - I260 184  Conditions of approved arrangement must not be contravened"@en-AU ;
    dct:isPartOf C2020A00012:259 ;
    dct:isReferencedBy C2020A00012: ;
    rdfs:comment "184  Conditions of approved arrangement must not be contravened - Abrievated Graph Key: I260"@en-AU ;
    skos:definition "184  Conditions of approved arrangement must not be contravened"@en-AU ;
    skos:narrower C2020A00012:259 ;
    skos:prefLabel "Item I260"@en-AU ;
    dcat:accessURL <https://www.legislation.gov.au/C2020A00012/2024-07-10/2024-07-10/text/original/epub/OEBPS/document_1/document_1.html#_Toc172118952> ;
    dcat:landingPage "https://www.legislation.gov.au/C2020A00012/2024-07-10/2024-07-10/text/original/epub/OEBPS/document_1/document_1.html#_Toc172118952"^^xsd:anyURI ;
    dcat:theme legcons:Item .

C2020A00012:261 a legcons:Item,
        owl:Class,
        dcat:Resource ;
    rdfs:label "Item - I261 185  Additional or corrected information in relation to application to approve proposed arrangement etc"@en-AU ;
    dct:isPartOf C2020A00012:259 ;
    dct:isReferencedBy C2020A00012: ;
    rdfs:comment "185  Additional or corrected information in relation to application to approve proposed arrangement etc - Abrievated Graph Key: I261"@en-AU ;
    skos:definition "185  Additional or corrected information in relation to application to approve proposed arrangement etc"@en-AU ;
    skos:narrower C2020A00012:259 ;
    skos:prefLabel "Item I261"@en-AU ;
    dcat:accessURL <https://www.legislation.gov.au/C2020A00012/2024-07-10/2024-07-10/text/original/epub/OEBPS/document_1/document_1.html#_Toc172118953> ;
    dcat:landingPage "https://www.legislation.gov.au/C2020A00012/2024-07-10/2024-07-10/text/original/epub/OEBPS/document_1/document_1.html#_Toc172118953"^^xsd:anyURI ;
    dcat:theme legcons:Item .

C2020A00012:262 a legcons:Item,
        owl:Class,
        dcat:Resource ;
    rdfs:label "Item - I262 186  Notice of changes to holder of approved arrangement"@en-AU ;
    dct:isPartOf C2020A00012:259 ;
    dct:isReferencedBy C2020A00012: ;
    rdfs:comment "186  Notice of changes to holder of approved arrangement - Abrievated Graph Key: I262"@en-AU ;
    skos:definition "186  Notice of changes to holder of approved arrangement"@en-AU ;
    skos:narrower C2020A00012:259 ;
    skos:prefLabel "Item I262"@en-AU ;
    dcat:accessURL <https://www.legislation.gov.au/C2020A00012/2024-07-10/2024-07-10/text/original/epub/OEBPS/document_1/document_1.html#_Toc172118954> ;
    dcat:landingPage "https://www.legislation.gov.au/C2020A00012/2024-07-10/2024-07-10/text/original/epub/OEBPS/document_1/document_1.html#_Toc172118954"^^xsd:anyURI ;
    dcat:theme legcons:Item .

C2020A00012:263 a legcons:Item,
        owl:Class,
        dcat:Resource ;
    rdfs:label "Item - I263 187  Notification of conviction of serious offence"@en-AU ;
    dct:isPartOf C2020A00012:259 ;
    dct:isReferencedBy C2020A00012: ;
    rdfs:comment "187  Notification of conviction of serious offence - Abrievated Graph Key: I263"@en-AU ;
    skos:definition "187  Notification of conviction of serious offence"@en-AU ;
    skos:narrower C2020A00012:259 ;
    skos:prefLabel "Item I263"@en-AU ;
    dcat:accessURL <https://www.legislation.gov.au/C2020A00012/2024-07-10/2024-07-10/text/original/epub/OEBPS/document_1/document_1.html#_Toc172118955> ;
    dcat:landingPage "https://www.legislation.gov.au/C2020A00012/2024-07-10/2024-07-10/text/original/epub/OEBPS/document_1/document_1.html#_Toc172118955"^^xsd:anyURI ;
    dcat:theme legcons:Item .

C2020A00012:264 a legcons:Item,
        owl:Class,
        dcat:Resource ;
    rdfs:label "Item - I264 188  Notice of person ceasing to operate business etc covered by approved arrangement"@en-AU ;
    dct:isPartOf C2020A00012:259 ;
    dct:isReferencedBy C2020A00012: ;
    rdfs:comment "188  Notice of person ceasing to operate business etc covered by approved arrangement - Abrievated Graph Key: I264"@en-AU ;
    skos:definition "188  Notice of person ceasing to operate business etc covered by approved arrangement"@en-AU ;
    skos:narrower C2020A00012:259 ;
    skos:prefLabel "Item I264"@en-AU ;
    dcat:accessURL <https://www.legislation.gov.au/C2020A00012/2024-07-10/2024-07-10/text/original/epub/OEBPS/document_1/document_1.html#_Toc172118956> ;
    dcat:landingPage "https://www.legislation.gov.au/C2020A00012/2024-07-10/2024-07-10/text/original/epub/OEBPS/document_1/document_1.html#_Toc172118956"^^xsd:anyURI ;
    dcat:theme legcons:Item .

C2020A00012:267 a legcons:Item,
        owl:Class,
        dcat:Resource ;
    rdfs:label "Item - I267 189  Simplified outline of this Chapter"@en-AU ;
    dct:isPartOf C2020A00012:266 ;
    dct:isReferencedBy C2020A00012: ;
    rdfs:comment "189  Simplified outline of this Chapter - Abrievated Graph Key: I267"@en-AU ;
    skos:definition "189  Simplified outline of this Chapter"@en-AU ;
    skos:narrower C2020A00012:266 ;
    skos:prefLabel "Item I267"@en-AU ;
    dcat:accessURL <https://www.legislation.gov.au/C2020A00012/2024-07-10/2024-07-10/text/original/epub/OEBPS/document_1/document_1.html#_Toc172118959> ;
    dcat:landingPage "https://www.legislation.gov.au/C2020A00012/2024-07-10/2024-07-10/text/original/epub/OEBPS/document_1/document_1.html#_Toc172118959"^^xsd:anyURI ;
    dcat:theme legcons:Item .

C2020A00012:269 a legcons:Item,
        owl:Class,
        dcat:Resource ;
    rdfs:label "Item - I269 190  Application for export licence"@en-AU ;
    dct:isPartOf C2020A00012:268 ;
    dct:isReferencedBy C2020A00012: ;
    rdfs:comment "190  Application for export licence - Abrievated Graph Key: I269"@en-AU ;
    skos:definition "190  Application for export licence"@en-AU ;
    skos:narrower C2020A00012:268 ;
    skos:prefLabel "Item I269"@en-AU ;
    dcat:accessURL <https://www.legislation.gov.au/C2020A00012/2024-07-10/2024-07-10/text/original/epub/OEBPS/document_1/document_1.html#_Toc172118961> ;
    dcat:landingPage "https://www.legislation.gov.au/C2020A00012/2024-07-10/2024-07-10/text/original/epub/OEBPS/document_1/document_1.html#_Toc172118961"^^xsd:anyURI ;
    dcat:theme legcons:Item .

C2020A00012:270 a legcons:Item,
        owl:Class,
        dcat:Resource ;
    rdfs:label "Item - I270 191  Secretary must decide whether to grant export licence"@en-AU ;
    dct:isPartOf C2020A00012:268 ;
    dct:isReferencedBy C2020A00012: ;
    rdfs:comment "191  Secretary must decide whether to grant export licence - Abrievated Graph Key: I270"@en-AU ;
    skos:definition "191  Secretary must decide whether to grant export licence"@en-AU ;
    skos:narrower C2020A00012:268 ;
    skos:prefLabel "Item I270"@en-AU ;
    dcat:accessURL <https://www.legislation.gov.au/C2020A00012/2024-07-10/2024-07-10/text/original/epub/OEBPS/document_1/document_1.html#_Toc172118962> ;
    dcat:landingPage "https://www.legislation.gov.au/C2020A00012/2024-07-10/2024-07-10/text/original/epub/OEBPS/document_1/document_1.html#_Toc172118962"^^xsd:anyURI ;
    dcat:theme legcons:Item .

C2020A00012:271 a legcons:Item,
        owl:Class,
        dcat:Resource ;
    rdfs:label "Item - I271 192  Conditions of export licence"@en-AU ;
    dct:isPartOf C2020A00012:268 ;
    dct:isReferencedBy C2020A00012: ;
    rdfs:comment "192  Conditions of export licence - Abrievated Graph Key: I271"@en-AU ;
    skos:definition "192  Conditions of export licence"@en-AU ;
    skos:narrower C2020A00012:268 ;
    skos:prefLabel "Item I271"@en-AU ;
    dcat:accessURL <https://www.legislation.gov.au/C2020A00012/2024-07-10/2024-07-10/text/original/epub/OEBPS/document_1/document_1.html#_Toc172118963> ;
    dcat:landingPage "https://www.legislation.gov.au/C2020A00012/2024-07-10/2024-07-10/text/original/epub/OEBPS/document_1/document_1.html#_Toc172118963"^^xsd:anyURI ;
    dcat:theme legcons:Item .

C2020A00012:272 a legcons:Item,
        owl:Class,
        dcat:Resource ;
    rdfs:label "Item - I272 193  Matters to be stated in export licence"@en-AU ;
    dct:isPartOf C2020A00012:268 ;
    dct:isReferencedBy C2020A00012: ;
    rdfs:comment "193  Matters to be stated in export licence - Abrievated Graph Key: I272"@en-AU ;
    skos:definition "193  Matters to be stated in export licence"@en-AU ;
    skos:narrower C2020A00012:268 ;
    skos:prefLabel "Item I272"@en-AU ;
    dcat:accessURL <https://www.legislation.gov.au/C2020A00012/2024-07-10/2024-07-10/text/original/epub/OEBPS/document_1/document_1.html#_Toc172118964> ;
    dcat:landingPage "https://www.legislation.gov.au/C2020A00012/2024-07-10/2024-07-10/text/original/epub/OEBPS/document_1/document_1.html#_Toc172118964"^^xsd:anyURI ;
    dcat:theme legcons:Item .

C2020A00012:273 a legcons:Item,
        owl:Class,
        dcat:Resource ;
    rdfs:label "Item - I273 194  Period of effect of export licence"@en-AU ;
    dct:isPartOf C2020A00012:268 ;
    dct:isReferencedBy C2020A00012: ;
    rdfs:comment "194  Period of effect of export licence - Abrievated Graph Key: I273"@en-AU ;
    skos:definition "194  Period of effect of export licence"@en-AU ;
    skos:narrower C2020A00012:268 ;
    skos:prefLabel "Item I273"@en-AU ;
    dcat:accessURL <https://www.legislation.gov.au/C2020A00012/2024-07-10/2024-07-10/text/original/epub/OEBPS/document_1/document_1.html#_Toc172118965> ;
    dcat:landingPage "https://www.legislation.gov.au/C2020A00012/2024-07-10/2024-07-10/text/original/epub/OEBPS/document_1/document_1.html#_Toc172118965"^^xsd:anyURI ;
    dcat:theme legcons:Item .

C2020A00012:275 a legcons:Item,
        owl:Class,
        dcat:Resource ;
    rdfs:label "Item - I275 195  Application to renew export licence"@en-AU ;
    dct:isPartOf C2020A00012:274 ;
    dct:isReferencedBy C2020A00012: ;
    rdfs:comment "195  Application to renew export licence - Abrievated Graph Key: I275"@en-AU ;
    skos:definition "195  Application to renew export licence"@en-AU ;
    skos:narrower C2020A00012:274 ;
    skos:prefLabel "Item I275"@en-AU ;
    dcat:accessURL <https://www.legislation.gov.au/C2020A00012/2024-07-10/2024-07-10/text/original/epub/OEBPS/document_1/document_1.html#_Toc172118967> ;
    dcat:landingPage "https://www.legislation.gov.au/C2020A00012/2024-07-10/2024-07-10/text/original/epub/OEBPS/document_1/document_1.html#_Toc172118967"^^xsd:anyURI ;
    dcat:theme legcons:Item .

C2020A00012:276 a legcons:Item,
        owl:Class,
        dcat:Resource ;
    rdfs:label "Item - I276 196  Secretary must decide whether to renew export licence"@en-AU ;
    dct:isPartOf C2020A00012:274 ;
    dct:isReferencedBy C2020A00012: ;
    rdfs:comment "196  Secretary must decide whether to renew export licence - Abrievated Graph Key: I276"@en-AU ;
    skos:definition "196  Secretary must decide whether to renew export licence"@en-AU ;
    skos:narrower C2020A00012:274 ;
    skos:prefLabel "Item I276"@en-AU ;
    dcat:accessURL <https://www.legislation.gov.au/C2020A00012/2024-07-10/2024-07-10/text/original/epub/OEBPS/document_1/document_1.html#_Toc172118968> ;
    dcat:landingPage "https://www.legislation.gov.au/C2020A00012/2024-07-10/2024-07-10/text/original/epub/OEBPS/document_1/document_1.html#_Toc172118968"^^xsd:anyURI ;
    dcat:theme legcons:Item .

C2020A00012:277 a legcons:Item,
        owl:Class,
        dcat:Resource ;
    rdfs:label "Item - I277 197  Conditions of renewed export licence"@en-AU ;
    dct:isPartOf C2020A00012:274 ;
    dct:isReferencedBy C2020A00012: ;
    rdfs:comment "197  Conditions of renewed export licence - Abrievated Graph Key: I277"@en-AU ;
    skos:definition "197  Conditions of renewed export licence"@en-AU ;
    skos:narrower C2020A00012:274 ;
    skos:prefLabel "Item I277"@en-AU ;
    dcat:accessURL <https://www.legislation.gov.au/C2020A00012/2024-07-10/2024-07-10/text/original/epub/OEBPS/document_1/document_1.html#_Toc172118969> ;
    dcat:landingPage "https://www.legislation.gov.au/C2020A00012/2024-07-10/2024-07-10/text/original/epub/OEBPS/document_1/document_1.html#_Toc172118969"^^xsd:anyURI ;
    dcat:theme legcons:Item .

C2020A00012:278 a legcons:Item,
        owl:Class,
        dcat:Resource ;
    rdfs:label "Item - I278 198  Matters to be stated in renewed export licence"@en-AU ;
    dct:isPartOf C2020A00012:274 ;
    dct:isReferencedBy C2020A00012: ;
    rdfs:comment "198  Matters to be stated in renewed export licence - Abrievated Graph Key: I278"@en-AU ;
    skos:definition "198  Matters to be stated in renewed export licence"@en-AU ;
    skos:narrower C2020A00012:274 ;
    skos:prefLabel "Item I278"@en-AU ;
    dcat:accessURL <https://www.legislation.gov.au/C2020A00012/2024-07-10/2024-07-10/text/original/epub/OEBPS/document_1/document_1.html#_Toc172118970> ;
    dcat:landingPage "https://www.legislation.gov.au/C2020A00012/2024-07-10/2024-07-10/text/original/epub/OEBPS/document_1/document_1.html#_Toc172118970"^^xsd:anyURI ;
    dcat:theme legcons:Item .

C2020A00012:281 a legcons:Item,
        owl:Class,
        dcat:Resource ;
    rdfs:label "Item - I281 199  Application by holder for variation of export licence"@en-AU ;
    dct:isPartOf C2020A00012:280 ;
    dct:isReferencedBy C2020A00012: ;
    rdfs:comment "199  Application by holder for variation of export licence - Abrievated Graph Key: I281"@en-AU ;
    skos:definition "199  Application by holder for variation of export licence"@en-AU ;
    skos:narrower C2020A00012:280 ;
    skos:prefLabel "Item I281"@en-AU ;
    dcat:accessURL <https://www.legislation.gov.au/C2020A00012/2024-07-10/2024-07-10/text/original/epub/OEBPS/document_1/document_1.html#_Toc172118973> ;
    dcat:landingPage "https://www.legislation.gov.au/C2020A00012/2024-07-10/2024-07-10/text/original/epub/OEBPS/document_1/document_1.html#_Toc172118973"^^xsd:anyURI ;
    dcat:theme legcons:Item .

C2020A00012:282 a legcons:Item,
        owl:Class,
        dcat:Resource ;
    rdfs:label "Item - I282 200  Notice of variation"@en-AU ;
    dct:isPartOf C2020A00012:280 ;
    dct:isReferencedBy C2020A00012: ;
    rdfs:comment "200  Notice of variation - Abrievated Graph Key: I282"@en-AU ;
    skos:definition "200  Notice of variation"@en-AU ;
    skos:narrower C2020A00012:280 ;
    skos:prefLabel "Item I282"@en-AU ;
    dcat:accessURL <https://www.legislation.gov.au/C2020A00012/2024-07-10/2024-07-10/text/original/epub/OEBPS/document_1/document_1.html#_Toc172118974> ;
    dcat:landingPage "https://www.legislation.gov.au/C2020A00012/2024-07-10/2024-07-10/text/original/epub/OEBPS/document_1/document_1.html#_Toc172118974"^^xsd:anyURI ;
    dcat:theme legcons:Item .

C2020A00012:284 a legcons:Item,
        owl:Class,
        dcat:Resource ;
    rdfs:label "Item - I284 201  Secretary may make variations in relation to export licence"@en-AU ;
    dct:isPartOf C2020A00012:283 ;
    dct:isReferencedBy C2020A00012: ;
    rdfs:comment "201  Secretary may make variations in relation to export licence - Abrievated Graph Key: I284"@en-AU ;
    skos:definition "201  Secretary may make variations in relation to export licence"@en-AU ;
    skos:narrower C2020A00012:283 ;
    skos:prefLabel "Item I284"@en-AU ;
    dcat:accessURL <https://www.legislation.gov.au/C2020A00012/2024-07-10/2024-07-10/text/original/epub/OEBPS/document_1/document_1.html#_Toc172118976> ;
    dcat:landingPage "https://www.legislation.gov.au/C2020A00012/2024-07-10/2024-07-10/text/original/epub/OEBPS/document_1/document_1.html#_Toc172118976"^^xsd:anyURI ;
    dcat:theme legcons:Item .

C2020A00012:285 a legcons:Item,
        owl:Class,
        dcat:Resource ;
    rdfs:label "Item - I285 202  Notice of variation"@en-AU ;
    dct:isPartOf C2020A00012:283 ;
    dct:isReferencedBy C2020A00012: ;
    rdfs:comment "202  Notice of variation - Abrievated Graph Key: I285"@en-AU ;
    skos:definition "202  Notice of variation"@en-AU ;
    skos:narrower C2020A00012:283 ;
    skos:prefLabel "Item I285"@en-AU ;
    dcat:accessURL <https://www.legislation.gov.au/C2020A00012/2024-07-10/2024-07-10/text/original/epub/OEBPS/document_1/document_1.html#_Toc172118977> ;
    dcat:landingPage "https://www.legislation.gov.au/C2020A00012/2024-07-10/2024-07-10/text/original/epub/OEBPS/document_1/document_1.html#_Toc172118977"^^xsd:anyURI ;
    dcat:theme legcons:Item .

C2020A00012:288 a legcons:Item,
        owl:Class,
        dcat:Resource ;
    rdfs:label "Item - I288 203  Holder may request suspension"@en-AU ;
    dct:isPartOf C2020A00012:287 ;
    dct:isReferencedBy C2020A00012: ;
    rdfs:comment "203  Holder may request suspension - Abrievated Graph Key: I288"@en-AU ;
    skos:definition "203  Holder may request suspension"@en-AU ;
    skos:narrower C2020A00012:287 ;
    skos:prefLabel "Item I288"@en-AU ;
    dcat:accessURL <https://www.legislation.gov.au/C2020A00012/2024-07-10/2024-07-10/text/original/epub/OEBPS/document_1/document_1.html#_Toc172118980> ;
    dcat:landingPage "https://www.legislation.gov.au/C2020A00012/2024-07-10/2024-07-10/text/original/epub/OEBPS/document_1/document_1.html#_Toc172118980"^^xsd:anyURI ;
    dcat:theme legcons:Item .

C2020A00012:289 a legcons:Item,
        owl:Class,
        dcat:Resource ;
    rdfs:label "Item - I289 204  Request to revoke suspension"@en-AU ;
    dct:isPartOf C2020A00012:287 ;
    dct:isReferencedBy C2020A00012: ;
    rdfs:comment "204  Request to revoke suspension - Abrievated Graph Key: I289"@en-AU ;
    skos:definition "204  Request to revoke suspension"@en-AU ;
    skos:narrower C2020A00012:287 ;
    skos:prefLabel "Item I289"@en-AU ;
    dcat:accessURL <https://www.legislation.gov.au/C2020A00012/2024-07-10/2024-07-10/text/original/epub/OEBPS/document_1/document_1.html#_Toc172118981> ;
    dcat:landingPage "https://www.legislation.gov.au/C2020A00012/2024-07-10/2024-07-10/text/original/epub/OEBPS/document_1/document_1.html#_Toc172118981"^^xsd:anyURI ;
    dcat:theme legcons:Item .

C2020A00012:291 a legcons:Item,
        owl:Class,
        dcat:Resource ;
    rdfs:label "Item - I291 205  Grounds for suspensiongeneral"@en-AU ;
    dct:isPartOf C2020A00012:290 ;
    dct:isReferencedBy C2020A00012: ;
    rdfs:comment "205  Grounds for suspensiongeneral - Abrievated Graph Key: I291"@en-AU ;
    skos:definition "205  Grounds for suspensiongeneral"@en-AU ;
    skos:narrower C2020A00012:290 ;
    skos:prefLabel "Item I291"@en-AU ;
    dcat:accessURL <https://www.legislation.gov.au/C2020A00012/2024-07-10/2024-07-10/text/original/epub/OEBPS/document_1/document_1.html#_Toc172118983> ;
    dcat:landingPage "https://www.legislation.gov.au/C2020A00012/2024-07-10/2024-07-10/text/original/epub/OEBPS/document_1/document_1.html#_Toc172118983"^^xsd:anyURI ;
    dcat:theme legcons:Item .

C2020A00012:292 a legcons:Item,
        owl:Class,
        dcat:Resource ;
    rdfs:label "Item - I292 206  Grounds for suspensionoverdue relevant Commonwealth liability"@en-AU ;
    dct:isPartOf C2020A00012:290 ;
    dct:isReferencedBy C2020A00012: ;
    rdfs:comment "206  Grounds for suspensionoverdue relevant Commonwealth liability - Abrievated Graph Key: I292"@en-AU ;
    skos:definition "206  Grounds for suspensionoverdue relevant Commonwealth liability"@en-AU ;
    skos:narrower C2020A00012:290 ;
    skos:prefLabel "Item I292"@en-AU ;
    dcat:accessURL <https://www.legislation.gov.au/C2020A00012/2024-07-10/2024-07-10/text/original/epub/OEBPS/document_1/document_1.html#_Toc172118984> ;
    dcat:landingPage "https://www.legislation.gov.au/C2020A00012/2024-07-10/2024-07-10/text/original/epub/OEBPS/document_1/document_1.html#_Toc172118984"^^xsd:anyURI ;
    dcat:theme legcons:Item .

C2020A00012:293 a legcons:Item,
        owl:Class,
        dcat:Resource ;
    rdfs:label "Item - I293 207  Notice of suspension"@en-AU ;
    dct:isPartOf C2020A00012:290 ;
    dct:isReferencedBy C2020A00012: ;
    rdfs:comment "207  Notice of suspension - Abrievated Graph Key: I293"@en-AU ;
    skos:definition "207  Notice of suspension"@en-AU ;
    skos:narrower C2020A00012:290 ;
    skos:prefLabel "Item I293"@en-AU ;
    dcat:accessURL <https://www.legislation.gov.au/C2020A00012/2024-07-10/2024-07-10/text/original/epub/OEBPS/document_1/document_1.html#_Toc172118985> ;
    dcat:landingPage "https://www.legislation.gov.au/C2020A00012/2024-07-10/2024-07-10/text/original/epub/OEBPS/document_1/document_1.html#_Toc172118985"^^xsd:anyURI ;
    dcat:theme legcons:Item .

C2020A00012:294 a legcons:Item,
        owl:Class,
        dcat:Resource ;
    rdfs:label "Item - I294 208  Period of suspension"@en-AU ;
    dct:isPartOf C2020A00012:290 ;
    dct:isReferencedBy C2020A00012: ;
    rdfs:comment "208  Period of suspension - Abrievated Graph Key: I294"@en-AU ;
    skos:definition "208  Period of suspension"@en-AU ;
    skos:narrower C2020A00012:290 ;
    skos:prefLabel "Item I294"@en-AU ;
    dcat:accessURL <https://www.legislation.gov.au/C2020A00012/2024-07-10/2024-07-10/text/original/epub/OEBPS/document_1/document_1.html#_Toc172118986> ;
    dcat:landingPage "https://www.legislation.gov.au/C2020A00012/2024-07-10/2024-07-10/text/original/epub/OEBPS/document_1/document_1.html#_Toc172118986"^^xsd:anyURI ;
    dcat:theme legcons:Item .

C2020A00012:295 a legcons:Item,
        owl:Class,
        dcat:Resource ;
    rdfs:label "Item - I295 209  Revocation of suspension"@en-AU ;
    dct:isPartOf C2020A00012:290 ;
    dct:isReferencedBy C2020A00012: ;
    rdfs:comment "209  Revocation of suspension - Abrievated Graph Key: I295"@en-AU ;
    skos:definition "209  Revocation of suspension"@en-AU ;
    skos:narrower C2020A00012:290 ;
    skos:prefLabel "Item I295"@en-AU ;
    dcat:accessURL <https://www.legislation.gov.au/C2020A00012/2024-07-10/2024-07-10/text/original/epub/OEBPS/document_1/document_1.html#_Toc172118987> ;
    dcat:landingPage "https://www.legislation.gov.au/C2020A00012/2024-07-10/2024-07-10/text/original/epub/OEBPS/document_1/document_1.html#_Toc172118987"^^xsd:anyURI ;
    dcat:theme legcons:Item .

C2020A00012:297 a legcons:Item,
        owl:Class,
        dcat:Resource ;
    rdfs:label "Item - I297 210  Effect of suspension"@en-AU ;
    dct:isPartOf C2020A00012:296 ;
    dct:isReferencedBy C2020A00012: ;
    rdfs:comment "210  Effect of suspension - Abrievated Graph Key: I297"@en-AU ;
    skos:definition "210  Effect of suspension"@en-AU ;
    skos:narrower C2020A00012:296 ;
    skos:prefLabel "Item I297"@en-AU ;
    dcat:accessURL <https://www.legislation.gov.au/C2020A00012/2024-07-10/2024-07-10/text/original/epub/OEBPS/document_1/document_1.html#_Toc172118989> ;
    dcat:landingPage "https://www.legislation.gov.au/C2020A00012/2024-07-10/2024-07-10/text/original/epub/OEBPS/document_1/document_1.html#_Toc172118989"^^xsd:anyURI ;
    dcat:theme legcons:Item .

C2020A00012:3 a legcons:Item,
        owl:Class,
        dcat:Resource ;
    rdfs:label "Item - I3 1  Short title"@en-AU ;
    dct:isPartOf C2020A00012:1 ;
    dct:isReferencedBy C2020A00012: ;
    rdfs:comment "1  Short title - Abrievated Graph Key: I3"@en-AU ;
    skos:definition "1  Short title"@en-AU ;
    skos:narrower C2020A00012:1 ;
    skos:prefLabel "Item I3"@en-AU ;
    dcat:accessURL <https://www.legislation.gov.au/C2020A00012/2024-07-10/2024-07-10/text/original/epub/OEBPS/document_1/document_1.html#_Toc172118695> ;
    dcat:landingPage "https://www.legislation.gov.au/C2020A00012/2024-07-10/2024-07-10/text/original/epub/OEBPS/document_1/document_1.html#_Toc172118695"^^xsd:anyURI ;
    dcat:theme legcons:Item .

C2020A00012:30 a legcons:Item,
        owl:Class,
        dcat:Resource ;
    rdfs:label "Item - I30 22  Simplified outline of this Part"@en-AU ;
    dct:isPartOf C2020A00012:29 ;
    dct:isReferencedBy C2020A00012: ;
    rdfs:comment "22  Simplified outline of this Part - Abrievated Graph Key: I30"@en-AU ;
    skos:definition "22  Simplified outline of this Part"@en-AU ;
    skos:narrower C2020A00012:29 ;
    skos:prefLabel "Item I30"@en-AU ;
    dcat:accessURL <https://www.legislation.gov.au/C2020A00012/2024-07-10/2024-07-10/text/original/epub/OEBPS/document_1/document_1.html#_Toc172118722> ;
    dcat:landingPage "https://www.legislation.gov.au/C2020A00012/2024-07-10/2024-07-10/text/original/epub/OEBPS/document_1/document_1.html#_Toc172118722"^^xsd:anyURI ;
    dcat:theme legcons:Item .

C2020A00012:300 a legcons:Item,
        owl:Class,
        dcat:Resource ;
    rdfs:label "Item - I300 211  Holder may request revocation"@en-AU ;
    dct:isPartOf C2020A00012:299 ;
    dct:isReferencedBy C2020A00012: ;
    rdfs:comment "211  Holder may request revocation - Abrievated Graph Key: I300"@en-AU ;
    skos:definition "211  Holder may request revocation"@en-AU ;
    skos:narrower C2020A00012:299 ;
    skos:prefLabel "Item I300"@en-AU ;
    dcat:accessURL <https://www.legislation.gov.au/C2020A00012/2024-07-10/2024-07-10/text/original/epub/OEBPS/document_1/document_1.html#_Toc172118992> ;
    dcat:landingPage "https://www.legislation.gov.au/C2020A00012/2024-07-10/2024-07-10/text/original/epub/OEBPS/document_1/document_1.html#_Toc172118992"^^xsd:anyURI ;
    dcat:theme legcons:Item .

C2020A00012:302 a legcons:Item,
        owl:Class,
        dcat:Resource ;
    rdfs:label "Item - I302 212  Grounds for revocationgeneral"@en-AU ;
    dct:isPartOf C2020A00012:301 ;
    dct:isReferencedBy C2020A00012: ;
    rdfs:comment "212  Grounds for revocationgeneral - Abrievated Graph Key: I302"@en-AU ;
    skos:definition "212  Grounds for revocationgeneral"@en-AU ;
    skos:narrower C2020A00012:301 ;
    skos:prefLabel "Item I302"@en-AU ;
    dcat:accessURL <https://www.legislation.gov.au/C2020A00012/2024-07-10/2024-07-10/text/original/epub/OEBPS/document_1/document_1.html#_Toc172118994> ;
    dcat:landingPage "https://www.legislation.gov.au/C2020A00012/2024-07-10/2024-07-10/text/original/epub/OEBPS/document_1/document_1.html#_Toc172118994"^^xsd:anyURI ;
    dcat:theme legcons:Item .

C2020A00012:303 a legcons:Item,
        owl:Class,
        dcat:Resource ;
    rdfs:label "Item - I303 213  Grounds for revocationoverdue relevant Commonwealth liability"@en-AU ;
    dct:isPartOf C2020A00012:301 ;
    dct:isReferencedBy C2020A00012: ;
    rdfs:comment "213  Grounds for revocationoverdue relevant Commonwealth liability - Abrievated Graph Key: I303"@en-AU ;
    skos:definition "213  Grounds for revocationoverdue relevant Commonwealth liability"@en-AU ;
    skos:narrower C2020A00012:301 ;
    skos:prefLabel "Item I303"@en-AU ;
    dcat:accessURL <https://www.legislation.gov.au/C2020A00012/2024-07-10/2024-07-10/text/original/epub/OEBPS/document_1/document_1.html#_Toc172118995> ;
    dcat:landingPage "https://www.legislation.gov.au/C2020A00012/2024-07-10/2024-07-10/text/original/epub/OEBPS/document_1/document_1.html#_Toc172118995"^^xsd:anyURI ;
    dcat:theme legcons:Item .

C2020A00012:304 a legcons:Item,
        owl:Class,
        dcat:Resource ;
    rdfs:label "Item - I304 214  Notice of revocation"@en-AU ;
    dct:isPartOf C2020A00012:301 ;
    dct:isReferencedBy C2020A00012: ;
    rdfs:comment "214  Notice of revocation - Abrievated Graph Key: I304"@en-AU ;
    skos:definition "214  Notice of revocation"@en-AU ;
    skos:narrower C2020A00012:301 ;
    skos:prefLabel "Item I304"@en-AU ;
    dcat:accessURL <https://www.legislation.gov.au/C2020A00012/2024-07-10/2024-07-10/text/original/epub/OEBPS/document_1/document_1.html#_Toc172118996> ;
    dcat:landingPage "https://www.legislation.gov.au/C2020A00012/2024-07-10/2024-07-10/text/original/epub/OEBPS/document_1/document_1.html#_Toc172118996"^^xsd:anyURI ;
    dcat:theme legcons:Item .

C2020A00012:306 a legcons:Item,
        owl:Class,
        dcat:Resource ;
    rdfs:label "Item - I306 215  Export operations must not be carried out after export licence revoked"@en-AU ;
    dct:isPartOf C2020A00012:305 ;
    dct:isReferencedBy C2020A00012: ;
    rdfs:comment "215  Export operations must not be carried out after export licence revoked - Abrievated Graph Key: I306"@en-AU ;
    skos:definition "215  Export operations must not be carried out after export licence revoked"@en-AU ;
    skos:narrower C2020A00012:305 ;
    skos:prefLabel "Item I306"@en-AU ;
    dcat:accessURL <https://www.legislation.gov.au/C2020A00012/2024-07-10/2024-07-10/text/original/epub/OEBPS/document_1/document_1.html#_Toc172118998> ;
    dcat:landingPage "https://www.legislation.gov.au/C2020A00012/2024-07-10/2024-07-10/text/original/epub/OEBPS/document_1/document_1.html#_Toc172118998"^^xsd:anyURI ;
    dcat:theme legcons:Item .

C2020A00012:307 a legcons:Item,
        owl:Class,
        dcat:Resource ;
    rdfs:label "Item - I307 216  Secretary may require action to be taken after export licence revoked"@en-AU ;
    dct:isPartOf C2020A00012:305 ;
    dct:isReferencedBy C2020A00012: ;
    rdfs:comment "216  Secretary may require action to be taken after export licence revoked - Abrievated Graph Key: I307"@en-AU ;
    skos:definition "216  Secretary may require action to be taken after export licence revoked"@en-AU ;
    skos:narrower C2020A00012:305 ;
    skos:prefLabel "Item I307"@en-AU ;
    dcat:accessURL <https://www.legislation.gov.au/C2020A00012/2024-07-10/2024-07-10/text/original/epub/OEBPS/document_1/document_1.html#_Toc172118999> ;
    dcat:landingPage "https://www.legislation.gov.au/C2020A00012/2024-07-10/2024-07-10/text/original/epub/OEBPS/document_1/document_1.html#_Toc172118999"^^xsd:anyURI ;
    dcat:theme legcons:Item .

C2020A00012:309 a legcons:Item,
        owl:Class,
        dcat:Resource ;
    rdfs:label "Item - I309 217  Conditions of export licence must not be contravened"@en-AU ;
    dct:isPartOf C2020A00012:308 ;
    dct:isReferencedBy C2020A00012: ;
    rdfs:comment "217  Conditions of export licence must not be contravened - Abrievated Graph Key: I309"@en-AU ;
    skos:definition "217  Conditions of export licence must not be contravened"@en-AU ;
    skos:narrower C2020A00012:308 ;
    skos:prefLabel "Item I309"@en-AU ;
    dcat:accessURL <https://www.legislation.gov.au/C2020A00012/2024-07-10/2024-07-10/text/original/epub/OEBPS/document_1/document_1.html#_Toc172119001> ;
    dcat:landingPage "https://www.legislation.gov.au/C2020A00012/2024-07-10/2024-07-10/text/original/epub/OEBPS/document_1/document_1.html#_Toc172119001"^^xsd:anyURI ;
    dcat:theme legcons:Item .

C2020A00012:310 a legcons:Item,
        owl:Class,
        dcat:Resource ;
    rdfs:label "Item - I310 218  Additional or corrected information in relation to application for licence etc"@en-AU ;
    dct:isPartOf C2020A00012:308 ;
    dct:isReferencedBy C2020A00012: ;
    rdfs:comment "218  Additional or corrected information in relation to application for licence etc - Abrievated Graph Key: I310"@en-AU ;
    skos:definition "218  Additional or corrected information in relation to application for licence etc"@en-AU ;
    skos:narrower C2020A00012:308 ;
    skos:prefLabel "Item I310"@en-AU ;
    dcat:accessURL <https://www.legislation.gov.au/C2020A00012/2024-07-10/2024-07-10/text/original/epub/OEBPS/document_1/document_1.html#_Toc172119002> ;
    dcat:landingPage "https://www.legislation.gov.au/C2020A00012/2024-07-10/2024-07-10/text/original/epub/OEBPS/document_1/document_1.html#_Toc172119002"^^xsd:anyURI ;
    dcat:theme legcons:Item .

C2020A00012:311 a legcons:Item,
        owl:Class,
        dcat:Resource ;
    rdfs:label "Item - I311 219  Notice of changes to holder of export licence"@en-AU ;
    dct:isPartOf C2020A00012:308 ;
    dct:isReferencedBy C2020A00012: ;
    rdfs:comment "219  Notice of changes to holder of export licence - Abrievated Graph Key: I311"@en-AU ;
    skos:definition "219  Notice of changes to holder of export licence"@en-AU ;
    skos:narrower C2020A00012:308 ;
    skos:prefLabel "Item I311"@en-AU ;
    dcat:accessURL <https://www.legislation.gov.au/C2020A00012/2024-07-10/2024-07-10/text/original/epub/OEBPS/document_1/document_1.html#_Toc172119003> ;
    dcat:landingPage "https://www.legislation.gov.au/C2020A00012/2024-07-10/2024-07-10/text/original/epub/OEBPS/document_1/document_1.html#_Toc172119003"^^xsd:anyURI ;
    dcat:theme legcons:Item .

C2020A00012:313 a legcons:Item,
        owl:Class,
        dcat:Resource ;
    rdfs:label "Item - I313 220  Persons who participate in the management or control of another persons export business"@en-AU ;
    dct:isPartOf C2020A00012:312 ;
    dct:isReferencedBy C2020A00012: ;
    rdfs:comment "220  Persons who participate in the management or control of another persons export business - Abrievated Graph Key: I313"@en-AU ;
    skos:definition "220  Persons who participate in the management or control of another persons export business"@en-AU ;
    skos:narrower C2020A00012:312 ;
    skos:prefLabel "Item I313"@en-AU ;
    dcat:accessURL <https://www.legislation.gov.au/C2020A00012/2024-07-10/2024-07-10/text/original/epub/OEBPS/document_1/document_1.html#_Toc172119005> ;
    dcat:landingPage "https://www.legislation.gov.au/C2020A00012/2024-07-10/2024-07-10/text/original/epub/OEBPS/document_1/document_1.html#_Toc172119005"^^xsd:anyURI ;
    dcat:theme legcons:Item .

C2020A00012:314 a legcons:Item,
        owl:Class,
        dcat:Resource ;
    rdfs:label "Item - I314 221  Secretarys powers in relation to associates of holder of export licence"@en-AU ;
    dct:isPartOf C2020A00012:312 ;
    dct:isReferencedBy C2020A00012: ;
    rdfs:comment "221  Secretarys powers in relation to associates of holder of export licence - Abrievated Graph Key: I314"@en-AU ;
    skos:definition "221  Secretarys powers in relation to associates of holder of export licence"@en-AU ;
    skos:narrower C2020A00012:312 ;
    skos:prefLabel "Item I314"@en-AU ;
    dcat:accessURL <https://www.legislation.gov.au/C2020A00012/2024-07-10/2024-07-10/text/original/epub/OEBPS/document_1/document_1.html#_Toc172119006> ;
    dcat:landingPage "https://www.legislation.gov.au/C2020A00012/2024-07-10/2024-07-10/text/original/epub/OEBPS/document_1/document_1.html#_Toc172119006"^^xsd:anyURI ;
    dcat:theme legcons:Item .

C2020A00012:315 a legcons:Item,
        owl:Class,
        dcat:Resource ;
    rdfs:label "Item - I315 222  Secretary may give directions to holder of export licence"@en-AU ;
    dct:isPartOf C2020A00012:312 ;
    dct:isReferencedBy C2020A00012: ;
    rdfs:comment "222  Secretary may give directions to holder of export licence - Abrievated Graph Key: I315"@en-AU ;
    skos:definition "222  Secretary may give directions to holder of export licence"@en-AU ;
    skos:narrower C2020A00012:312 ;
    skos:prefLabel "Item I315"@en-AU ;
    dcat:accessURL <https://www.legislation.gov.au/C2020A00012/2024-07-10/2024-07-10/text/original/epub/OEBPS/document_1/document_1.html#_Toc172119007> ;
    dcat:landingPage "https://www.legislation.gov.au/C2020A00012/2024-07-10/2024-07-10/text/original/epub/OEBPS/document_1/document_1.html#_Toc172119007"^^xsd:anyURI ;
    dcat:theme legcons:Item .

C2020A00012:318 a legcons:Item,
        owl:Class,
        dcat:Resource ;
    rdfs:label "Item - I318 223  Simplified outline of this Chapter"@en-AU ;
    dct:isPartOf C2020A00012:317 ;
    dct:isReferencedBy C2020A00012: ;
    rdfs:comment "223  Simplified outline of this Chapter - Abrievated Graph Key: I318"@en-AU ;
    skos:definition "223  Simplified outline of this Chapter"@en-AU ;
    skos:narrower C2020A00012:317 ;
    skos:prefLabel "Item I318"@en-AU ;
    dcat:accessURL <https://www.legislation.gov.au/C2020A00012/2024-07-10/2024-07-10/text/original/epub/OEBPS/document_1/document_1.html#_Toc172119010> ;
    dcat:landingPage "https://www.legislation.gov.au/C2020A00012/2024-07-10/2024-07-10/text/original/epub/OEBPS/document_1/document_1.html#_Toc172119010"^^xsd:anyURI ;
    dcat:theme legcons:Item .

C2020A00012:320 a legcons:Item,
        owl:Class,
        dcat:Resource ;
    rdfs:label "Item - I320 224  Application for export permit"@en-AU ;
    dct:isPartOf C2020A00012:319 ;
    dct:isReferencedBy C2020A00012: ;
    rdfs:comment "224  Application for export permit - Abrievated Graph Key: I320"@en-AU ;
    skos:definition "224  Application for export permit"@en-AU ;
    skos:narrower C2020A00012:319 ;
    skos:prefLabel "Item I320"@en-AU ;
    dcat:accessURL <https://www.legislation.gov.au/C2020A00012/2024-07-10/2024-07-10/text/original/epub/OEBPS/document_1/document_1.html#_Toc172119012> ;
    dcat:landingPage "https://www.legislation.gov.au/C2020A00012/2024-07-10/2024-07-10/text/original/epub/OEBPS/document_1/document_1.html#_Toc172119012"^^xsd:anyURI ;
    dcat:theme legcons:Item .

C2020A00012:321 a legcons:Item,
        owl:Class,
        dcat:Resource ;
    rdfs:label "Item - I321 225  Secretary must decide whether to issue export permit"@en-AU ;
    dct:isPartOf C2020A00012:319 ;
    dct:isReferencedBy C2020A00012: ;
    rdfs:comment "225  Secretary must decide whether to issue export permit - Abrievated Graph Key: I321"@en-AU ;
    skos:definition "225  Secretary must decide whether to issue export permit"@en-AU ;
    skos:narrower C2020A00012:319 ;
    skos:prefLabel "Item I321"@en-AU ;
    dcat:accessURL <https://www.legislation.gov.au/C2020A00012/2024-07-10/2024-07-10/text/original/epub/OEBPS/document_1/document_1.html#_Toc172119013> ;
    dcat:landingPage "https://www.legislation.gov.au/C2020A00012/2024-07-10/2024-07-10/text/original/epub/OEBPS/document_1/document_1.html#_Toc172119013"^^xsd:anyURI ;
    dcat:theme legcons:Item .

C2020A00012:322 a legcons:Item,
        owl:Class,
        dcat:Resource ;
    rdfs:label "Item - I322 226  Requirements for export permit"@en-AU ;
    dct:isPartOf C2020A00012:319 ;
    dct:isReferencedBy C2020A00012: ;
    rdfs:comment "226  Requirements for export permit - Abrievated Graph Key: I322"@en-AU ;
    skos:definition "226  Requirements for export permit"@en-AU ;
    skos:narrower C2020A00012:319 ;
    skos:prefLabel "Item I322"@en-AU ;
    dcat:accessURL <https://www.legislation.gov.au/C2020A00012/2024-07-10/2024-07-10/text/original/epub/OEBPS/document_1/document_1.html#_Toc172119014> ;
    dcat:landingPage "https://www.legislation.gov.au/C2020A00012/2024-07-10/2024-07-10/text/original/epub/OEBPS/document_1/document_1.html#_Toc172119014"^^xsd:anyURI ;
    dcat:theme legcons:Item .

C2020A00012:323 a legcons:Item,
        owl:Class,
        dcat:Resource ;
    rdfs:label "Item - I323 227  Conditions of export permit"@en-AU ;
    dct:isPartOf C2020A00012:319 ;
    dct:isReferencedBy C2020A00012: ;
    rdfs:comment "227  Conditions of export permit - Abrievated Graph Key: I323"@en-AU ;
    skos:definition "227  Conditions of export permit"@en-AU ;
    skos:narrower C2020A00012:319 ;
    skos:prefLabel "Item I323"@en-AU ;
    dcat:accessURL <https://www.legislation.gov.au/C2020A00012/2024-07-10/2024-07-10/text/original/epub/OEBPS/document_1/document_1.html#_Toc172119015> ;
    dcat:landingPage "https://www.legislation.gov.au/C2020A00012/2024-07-10/2024-07-10/text/original/epub/OEBPS/document_1/document_1.html#_Toc172119015"^^xsd:anyURI ;
    dcat:theme legcons:Item .

C2020A00012:324 a legcons:Item,
        owl:Class,
        dcat:Resource ;
    rdfs:label "Item - I324 228  Period of effect of export permit"@en-AU ;
    dct:isPartOf C2020A00012:319 ;
    dct:isReferencedBy C2020A00012: ;
    rdfs:comment "228  Period of effect of export permit - Abrievated Graph Key: I324"@en-AU ;
    skos:definition "228  Period of effect of export permit"@en-AU ;
    skos:narrower C2020A00012:319 ;
    skos:prefLabel "Item I324"@en-AU ;
    dcat:accessURL <https://www.legislation.gov.au/C2020A00012/2024-07-10/2024-07-10/text/original/epub/OEBPS/document_1/document_1.html#_Toc172119016> ;
    dcat:landingPage "https://www.legislation.gov.au/C2020A00012/2024-07-10/2024-07-10/text/original/epub/OEBPS/document_1/document_1.html#_Toc172119016"^^xsd:anyURI ;
    dcat:theme legcons:Item .

C2020A00012:326 a legcons:Item,
        owl:Class,
        dcat:Resource ;
    rdfs:label "Item - I326 229  Secretary may vary export permit or conditions of permit"@en-AU ;
    dct:isPartOf C2020A00012:325 ;
    dct:isReferencedBy C2020A00012: ;
    rdfs:comment "229  Secretary may vary export permit or conditions of permit - Abrievated Graph Key: I326"@en-AU ;
    skos:definition "229  Secretary may vary export permit or conditions of permit"@en-AU ;
    skos:narrower C2020A00012:325 ;
    skos:prefLabel "Item I326"@en-AU ;
    dcat:accessURL <https://www.legislation.gov.au/C2020A00012/2024-07-10/2024-07-10/text/original/epub/OEBPS/document_1/document_1.html#_Toc172119018> ;
    dcat:landingPage "https://www.legislation.gov.au/C2020A00012/2024-07-10/2024-07-10/text/original/epub/OEBPS/document_1/document_1.html#_Toc172119018"^^xsd:anyURI ;
    dcat:theme legcons:Item .

C2020A00012:327 a legcons:Item,
        owl:Class,
        dcat:Resource ;
    rdfs:label "Item - I327 230  Period of effect of varied export permit"@en-AU ;
    dct:isPartOf C2020A00012:325 ;
    dct:isReferencedBy C2020A00012: ;
    rdfs:comment "230  Period of effect of varied export permit - Abrievated Graph Key: I327"@en-AU ;
    skos:definition "230  Period of effect of varied export permit"@en-AU ;
    skos:narrower C2020A00012:325 ;
    skos:prefLabel "Item I327"@en-AU ;
    dcat:accessURL <https://www.legislation.gov.au/C2020A00012/2024-07-10/2024-07-10/text/original/epub/OEBPS/document_1/document_1.html#_Toc172119019> ;
    dcat:landingPage "https://www.legislation.gov.au/C2020A00012/2024-07-10/2024-07-10/text/original/epub/OEBPS/document_1/document_1.html#_Toc172119019"^^xsd:anyURI ;
    dcat:theme legcons:Item .

C2020A00012:328 a legcons:Item,
        owl:Class,
        dcat:Resource ;
    rdfs:label "Item - I328 231  Secretary may suspend export permit"@en-AU ;
    dct:isPartOf C2020A00012:325 ;
    dct:isReferencedBy C2020A00012: ;
    rdfs:comment "231  Secretary may suspend export permit - Abrievated Graph Key: I328"@en-AU ;
    skos:definition "231  Secretary may suspend export permit"@en-AU ;
    skos:narrower C2020A00012:325 ;
    skos:prefLabel "Item I328"@en-AU ;
    dcat:accessURL <https://www.legislation.gov.au/C2020A00012/2024-07-10/2024-07-10/text/original/epub/OEBPS/document_1/document_1.html#_Toc172119020> ;
    dcat:landingPage "https://www.legislation.gov.au/C2020A00012/2024-07-10/2024-07-10/text/original/epub/OEBPS/document_1/document_1.html#_Toc172119020"^^xsd:anyURI ;
    dcat:theme legcons:Item .

C2020A00012:329 a legcons:Item,
        owl:Class,
        dcat:Resource ;
    rdfs:label "Item - I329 232  Effect of suspension"@en-AU ;
    dct:isPartOf C2020A00012:325 ;
    dct:isReferencedBy C2020A00012: ;
    rdfs:comment "232  Effect of suspension - Abrievated Graph Key: I329"@en-AU ;
    skos:definition "232  Effect of suspension"@en-AU ;
    skos:narrower C2020A00012:325 ;
    skos:prefLabel "Item I329"@en-AU ;
    dcat:accessURL <https://www.legislation.gov.au/C2020A00012/2024-07-10/2024-07-10/text/original/epub/OEBPS/document_1/document_1.html#_Toc172119021> ;
    dcat:landingPage "https://www.legislation.gov.au/C2020A00012/2024-07-10/2024-07-10/text/original/epub/OEBPS/document_1/document_1.html#_Toc172119021"^^xsd:anyURI ;
    dcat:theme legcons:Item .

C2020A00012:33 a legcons:Item,
        owl:Class,
        dcat:Resource ;
    rdfs:label "Item - I33 23  Goods that are prohibited from export absolutely"@en-AU ;
    dct:isPartOf C2020A00012:32 ;
    dct:isReferencedBy C2020A00012: ;
    rdfs:comment "23  Goods that are prohibited from export absolutely - Abrievated Graph Key: I33"@en-AU ;
    skos:definition "23  Goods that are prohibited from export absolutely"@en-AU ;
    skos:narrower C2020A00012:32 ;
    skos:prefLabel "Item I33"@en-AU ;
    dcat:accessURL <https://www.legislation.gov.au/C2020A00012/2024-07-10/2024-07-10/text/original/epub/OEBPS/document_1/document_1.html#_Toc172118725> ;
    dcat:landingPage "https://www.legislation.gov.au/C2020A00012/2024-07-10/2024-07-10/text/original/epub/OEBPS/document_1/document_1.html#_Toc172118725"^^xsd:anyURI ;
    dcat:theme legcons:Item .

C2020A00012:330 a legcons:Item,
        owl:Class,
        dcat:Resource ;
    rdfs:label "Item - I330 233  Secretary may revoke export permit"@en-AU ;
    dct:isPartOf C2020A00012:325 ;
    dct:isReferencedBy C2020A00012: ;
    rdfs:comment "233  Secretary may revoke export permit - Abrievated Graph Key: I330"@en-AU ;
    skos:definition "233  Secretary may revoke export permit"@en-AU ;
    skos:narrower C2020A00012:325 ;
    skos:prefLabel "Item I330"@en-AU ;
    dcat:accessURL <https://www.legislation.gov.au/C2020A00012/2024-07-10/2024-07-10/text/original/epub/OEBPS/document_1/document_1.html#_Toc172119022> ;
    dcat:landingPage "https://www.legislation.gov.au/C2020A00012/2024-07-10/2024-07-10/text/original/epub/OEBPS/document_1/document_1.html#_Toc172119022"^^xsd:anyURI ;
    dcat:theme legcons:Item .

C2020A00012:332 a legcons:Item,
        owl:Class,
        dcat:Resource ;
    rdfs:label "Item - I332 234  Secretary may require assessment of goods"@en-AU ;
    dct:isPartOf C2020A00012:331 ;
    dct:isReferencedBy C2020A00012: ;
    rdfs:comment "234  Secretary may require assessment of goods - Abrievated Graph Key: I332"@en-AU ;
    skos:definition "234  Secretary may require assessment of goods"@en-AU ;
    skos:narrower C2020A00012:331 ;
    skos:prefLabel "Item I332"@en-AU ;
    dcat:accessURL <https://www.legislation.gov.au/C2020A00012/2024-07-10/2024-07-10/text/original/epub/OEBPS/document_1/document_1.html#_Toc172119024> ;
    dcat:landingPage "https://www.legislation.gov.au/C2020A00012/2024-07-10/2024-07-10/text/original/epub/OEBPS/document_1/document_1.html#_Toc172119024"^^xsd:anyURI ;
    dcat:theme legcons:Item .

C2020A00012:333 a legcons:Item,
        owl:Class,
        dcat:Resource ;
    rdfs:label "Item - I333 235  Additional or corrected information in relation to application for export permit etc"@en-AU ;
    dct:isPartOf C2020A00012:331 ;
    dct:isReferencedBy C2020A00012: ;
    rdfs:comment "235  Additional or corrected information in relation to application for export permit etc - Abrievated Graph Key: I333"@en-AU ;
    skos:definition "235  Additional or corrected information in relation to application for export permit etc"@en-AU ;
    skos:narrower C2020A00012:331 ;
    skos:prefLabel "Item I333"@en-AU ;
    dcat:accessURL <https://www.legislation.gov.au/C2020A00012/2024-07-10/2024-07-10/text/original/epub/OEBPS/document_1/document_1.html#_Toc172119025> ;
    dcat:landingPage "https://www.legislation.gov.au/C2020A00012/2024-07-10/2024-07-10/text/original/epub/OEBPS/document_1/document_1.html#_Toc172119025"^^xsd:anyURI ;
    dcat:theme legcons:Item .

C2020A00012:334 a legcons:Item,
        owl:Class,
        dcat:Resource ;
    rdfs:label "Item - I334 236  Return of export permit"@en-AU ;
    dct:isPartOf C2020A00012:331 ;
    dct:isReferencedBy C2020A00012: ;
    rdfs:comment "236  Return of export permit - Abrievated Graph Key: I334"@en-AU ;
    skos:definition "236  Return of export permit"@en-AU ;
    skos:narrower C2020A00012:331 ;
    skos:prefLabel "Item I334"@en-AU ;
    dcat:accessURL <https://www.legislation.gov.au/C2020A00012/2024-07-10/2024-07-10/text/original/epub/OEBPS/document_1/document_1.html#_Toc172119026> ;
    dcat:landingPage "https://www.legislation.gov.au/C2020A00012/2024-07-10/2024-07-10/text/original/epub/OEBPS/document_1/document_1.html#_Toc172119026"^^xsd:anyURI ;
    dcat:theme legcons:Item .

C2020A00012:335 a legcons:Item,
        owl:Class,
        dcat:Resource ;
    rdfs:label "Item - I335 237  Notification that goods not to be exported"@en-AU ;
    dct:isPartOf C2020A00012:331 ;
    dct:isReferencedBy C2020A00012: ;
    rdfs:comment "237  Notification that goods not to be exported - Abrievated Graph Key: I335"@en-AU ;
    skos:definition "237  Notification that goods not to be exported"@en-AU ;
    skos:narrower C2020A00012:331 ;
    skos:prefLabel "Item I335"@en-AU ;
    dcat:accessURL <https://www.legislation.gov.au/C2020A00012/2024-07-10/2024-07-10/text/original/epub/OEBPS/document_1/document_1.html#_Toc172119027> ;
    dcat:landingPage "https://www.legislation.gov.au/C2020A00012/2024-07-10/2024-07-10/text/original/epub/OEBPS/document_1/document_1.html#_Toc172119027"^^xsd:anyURI ;
    dcat:theme legcons:Item .

C2020A00012:337 a legcons:Item,
        owl:Class,
        dcat:Resource ;
    rdfs:label "Item - I337 238  Applications to which this Part applies"@en-AU ;
    dct:isPartOf C2020A00012:336 ;
    dct:isReferencedBy C2020A00012: ;
    rdfs:comment "238  Applications to which this Part applies - Abrievated Graph Key: I337"@en-AU ;
    skos:definition "238  Applications to which this Part applies"@en-AU ;
    skos:narrower C2020A00012:336 ;
    skos:prefLabel "Item I337"@en-AU ;
    dcat:accessURL <https://www.legislation.gov.au/C2020A00012/2024-07-10/2024-07-10/text/original/epub/OEBPS/document_1/document_1.html#_Toc172119029> ;
    dcat:landingPage "https://www.legislation.gov.au/C2020A00012/2024-07-10/2024-07-10/text/original/epub/OEBPS/document_1/document_1.html#_Toc172119029"^^xsd:anyURI ;
    dcat:theme legcons:Item .

C2020A00012:338 a legcons:Item,
        owl:Class,
        dcat:Resource ;
    rdfs:label "Item - I338 239  Requirements for applications"@en-AU ;
    dct:isPartOf C2020A00012:336 ;
    dct:isReferencedBy C2020A00012: ;
    rdfs:comment "239  Requirements for applications - Abrievated Graph Key: I338"@en-AU ;
    skos:definition "239  Requirements for applications"@en-AU ;
    skos:narrower C2020A00012:336 ;
    skos:prefLabel "Item I338"@en-AU ;
    dcat:accessURL <https://www.legislation.gov.au/C2020A00012/2024-07-10/2024-07-10/text/original/epub/OEBPS/document_1/document_1.html#_Toc172119030> ;
    dcat:landingPage "https://www.legislation.gov.au/C2020A00012/2024-07-10/2024-07-10/text/original/epub/OEBPS/document_1/document_1.html#_Toc172119030"^^xsd:anyURI ;
    dcat:theme legcons:Item .

C2020A00012:339 a legcons:Item,
        owl:Class,
        dcat:Resource ;
    rdfs:label "Item - I339 240  Additional or corrected information"@en-AU ;
    dct:isPartOf C2020A00012:336 ;
    dct:isReferencedBy C2020A00012: ;
    rdfs:comment "240  Additional or corrected information - Abrievated Graph Key: I339"@en-AU ;
    skos:definition "240  Additional or corrected information"@en-AU ;
    skos:narrower C2020A00012:336 ;
    skos:prefLabel "Item I339"@en-AU ;
    dcat:accessURL <https://www.legislation.gov.au/C2020A00012/2024-07-10/2024-07-10/text/original/epub/OEBPS/document_1/document_1.html#_Toc172119031> ;
    dcat:landingPage "https://www.legislation.gov.au/C2020A00012/2024-07-10/2024-07-10/text/original/epub/OEBPS/document_1/document_1.html#_Toc172119031"^^xsd:anyURI ;
    dcat:theme legcons:Item .

C2020A00012:34 a legcons:Item,
        owl:Class,
        dcat:Resource ;
    rdfs:label "Item - I34 23 A  Goods that are prohibited from export by sea"@en-AU ;
    dct:isPartOf C2020A00012:32 ;
    dct:isReferencedBy C2020A00012: ;
    rdfs:comment "23 A  Goods that are prohibited from export by sea - Abrievated Graph Key: I34"@en-AU ;
    skos:definition "23 A  Goods that are prohibited from export by sea"@en-AU ;
    skos:narrower C2020A00012:32 ;
    skos:prefLabel "Item I34"@en-AU ;
    dcat:accessURL <https://www.legislation.gov.au/C2020A00012/2024-07-10/2024-07-10/text/original/epub/OEBPS/document_1/document_1.html#_Toc172118726> ;
    dcat:landingPage "https://www.legislation.gov.au/C2020A00012/2024-07-10/2024-07-10/text/original/epub/OEBPS/document_1/document_1.html#_Toc172118726"^^xsd:anyURI ;
    dcat:theme legcons:Item .

C2020A00012:340 a legcons:Item,
        owl:Class,
        dcat:Resource ;
    rdfs:label "Item - I340 241  Powers of Secretary in relation to application"@en-AU ;
    dct:isPartOf C2020A00012:336 ;
    dct:isReferencedBy C2020A00012: ;
    rdfs:comment "241  Powers of Secretary in relation to application - Abrievated Graph Key: I340"@en-AU ;
    skos:definition "241  Powers of Secretary in relation to application"@en-AU ;
    skos:narrower C2020A00012:336 ;
    skos:prefLabel "Item I340"@en-AU ;
    dcat:accessURL <https://www.legislation.gov.au/C2020A00012/2024-07-10/2024-07-10/text/original/epub/OEBPS/document_1/document_1.html#_Toc172119032> ;
    dcat:landingPage "https://www.legislation.gov.au/C2020A00012/2024-07-10/2024-07-10/text/original/epub/OEBPS/document_1/document_1.html#_Toc172119032"^^xsd:anyURI ;
    dcat:theme legcons:Item .

C2020A00012:344 a legcons:Item,
        owl:Class,
        dcat:Resource ;
    rdfs:label "Item - I344 242  Simplified outline of this Part"@en-AU ;
    dct:isPartOf C2020A00012:343 ;
    dct:isReferencedBy C2020A00012: ;
    rdfs:comment "242  Simplified outline of this Part - Abrievated Graph Key: I344"@en-AU ;
    skos:definition "242  Simplified outline of this Part"@en-AU ;
    skos:narrower C2020A00012:343 ;
    skos:prefLabel "Item I344"@en-AU ;
    dcat:accessURL <https://www.legislation.gov.au/C2020A00012/2024-07-10/2024-07-10/text/original/epub/OEBPS/document_1/document_1.html#_Toc172119036> ;
    dcat:landingPage "https://www.legislation.gov.au/C2020A00012/2024-07-10/2024-07-10/text/original/epub/OEBPS/document_1/document_1.html#_Toc172119036"^^xsd:anyURI ;
    dcat:theme legcons:Item .

C2020A00012:346 a legcons:Item,
        owl:Class,
        dcat:Resource ;
    rdfs:label "Item - I346 243  Notice of intention to exportgeneral"@en-AU ;
    dct:isPartOf C2020A00012:345 ;
    dct:isReferencedBy C2020A00012: ;
    rdfs:comment "243  Notice of intention to exportgeneral - Abrievated Graph Key: I346"@en-AU ;
    skos:definition "243  Notice of intention to exportgeneral"@en-AU ;
    skos:narrower C2020A00012:345 ;
    skos:prefLabel "Item I346"@en-AU ;
    dcat:accessURL <https://www.legislation.gov.au/C2020A00012/2024-07-10/2024-07-10/text/original/epub/OEBPS/document_1/document_1.html#_Toc172119038> ;
    dcat:landingPage "https://www.legislation.gov.au/C2020A00012/2024-07-10/2024-07-10/text/original/epub/OEBPS/document_1/document_1.html#_Toc172119038"^^xsd:anyURI ;
    dcat:theme legcons:Item .

C2020A00012:347 a legcons:Item,
        owl:Class,
        dcat:Resource ;
    rdfs:label "Item - I347 244  Additional or corrected information"@en-AU ;
    dct:isPartOf C2020A00012:345 ;
    dct:isReferencedBy C2020A00012: ;
    rdfs:comment "244  Additional or corrected information - Abrievated Graph Key: I347"@en-AU ;
    skos:definition "244  Additional or corrected information"@en-AU ;
    skos:narrower C2020A00012:345 ;
    skos:prefLabel "Item I347"@en-AU ;
    dcat:accessURL <https://www.legislation.gov.au/C2020A00012/2024-07-10/2024-07-10/text/original/epub/OEBPS/document_1/document_1.html#_Toc172119039> ;
    dcat:landingPage "https://www.legislation.gov.au/C2020A00012/2024-07-10/2024-07-10/text/original/epub/OEBPS/document_1/document_1.html#_Toc172119039"^^xsd:anyURI ;
    dcat:theme legcons:Item .

C2020A00012:35 a legcons:Subdivision,
        owl:Class,
        dcat:Resource ;
    rdfs:label "Subdivision - S35 Subdivision BTemporarily prohibited goods"@en-AU ;
    dct:isPartOf C2020A00012:31 ;
    dct:isReferencedBy C2020A00012: ;
    rdfs:comment "Subdivision BTemporarily prohibited goods - Abrievated Graph Key: S35"@en-AU ;
    skos:definition "Subdivision BTemporarily prohibited goods"@en-AU ;
    skos:narrower C2020A00012:31 ;
    skos:prefLabel "Subdivision S35"@en-AU ;
    dcat:accessURL <https://www.legislation.gov.au/C2020A00012/2024-07-10/2024-07-10/text/original/epub/OEBPS/document_1/document_1.html#_Toc172118727> ;
    dcat:landingPage "https://www.legislation.gov.au/C2020A00012/2024-07-10/2024-07-10/text/original/epub/OEBPS/document_1/document_1.html#_Toc172118727"^^xsd:anyURI ;
    dcat:theme legcons:Subdivision .

C2020A00012:350 a legcons:Item,
        owl:Class,
        dcat:Resource ;
    rdfs:label "Item - I350 245  Simplified outline of this Part"@en-AU ;
    dct:isPartOf C2020A00012:349 ;
    dct:isReferencedBy C2020A00012: ;
    rdfs:comment "245  Simplified outline of this Part - Abrievated Graph Key: I350"@en-AU ;
    skos:definition "245  Simplified outline of this Part"@en-AU ;
    skos:narrower C2020A00012:349 ;
    skos:prefLabel "Item I350"@en-AU ;
    dcat:accessURL <https://www.legislation.gov.au/C2020A00012/2024-07-10/2024-07-10/text/original/epub/OEBPS/document_1/document_1.html#_Toc172119042> ;
    dcat:landingPage "https://www.legislation.gov.au/C2020A00012/2024-07-10/2024-07-10/text/original/epub/OEBPS/document_1/document_1.html#_Toc172119042"^^xsd:anyURI ;
    dcat:theme legcons:Item .

C2020A00012:352 a legcons:Item,
        owl:Class,
        dcat:Resource ;
    rdfs:label "Item - I352 246  Meaning of trade description"@en-AU ;
    dct:isPartOf C2020A00012:351 ;
    dct:isReferencedBy C2020A00012: ;
    rdfs:comment "246  Meaning of trade description - Abrievated Graph Key: I352"@en-AU ;
    skos:definition "246  Meaning of trade description"@en-AU ;
    skos:narrower C2020A00012:351 ;
    skos:prefLabel "Item I352"@en-AU ;
    dcat:accessURL <https://www.legislation.gov.au/C2020A00012/2024-07-10/2024-07-10/text/original/epub/OEBPS/document_1/document_1.html#_Toc172119044> ;
    dcat:landingPage "https://www.legislation.gov.au/C2020A00012/2024-07-10/2024-07-10/text/original/epub/OEBPS/document_1/document_1.html#_Toc172119044"^^xsd:anyURI ;
    dcat:theme legcons:Item .

C2020A00012:353 a legcons:Item,
        owl:Class,
        dcat:Resource ;
    rdfs:label "Item - I353 247  When a trade description is applied to goods"@en-AU ;
    dct:isPartOf C2020A00012:351 ;
    dct:isReferencedBy C2020A00012: ;
    rdfs:comment "247  When a trade description is applied to goods - Abrievated Graph Key: I353"@en-AU ;
    skos:definition "247  When a trade description is applied to goods"@en-AU ;
    skos:narrower C2020A00012:351 ;
    skos:prefLabel "Item I353"@en-AU ;
    dcat:accessURL <https://www.legislation.gov.au/C2020A00012/2024-07-10/2024-07-10/text/original/epub/OEBPS/document_1/document_1.html#_Toc172119045> ;
    dcat:landingPage "https://www.legislation.gov.au/C2020A00012/2024-07-10/2024-07-10/text/original/epub/OEBPS/document_1/document_1.html#_Toc172119045"^^xsd:anyURI ;
    dcat:theme legcons:Item .

C2020A00012:354 a legcons:Item,
        owl:Class,
        dcat:Resource ;
    rdfs:label "Item - I354 248  Rules may make provision in relation to trade descriptions"@en-AU ;
    dct:isPartOf C2020A00012:351 ;
    dct:isReferencedBy C2020A00012: ;
    rdfs:comment "248  Rules may make provision in relation to trade descriptions - Abrievated Graph Key: I354"@en-AU ;
    skos:definition "248  Rules may make provision in relation to trade descriptions"@en-AU ;
    skos:narrower C2020A00012:351 ;
    skos:prefLabel "Item I354"@en-AU ;
    dcat:accessURL <https://www.legislation.gov.au/C2020A00012/2024-07-10/2024-07-10/text/original/epub/OEBPS/document_1/document_1.html#_Toc172119046> ;
    dcat:landingPage "https://www.legislation.gov.au/C2020A00012/2024-07-10/2024-07-10/text/original/epub/OEBPS/document_1/document_1.html#_Toc172119046"^^xsd:anyURI ;
    dcat:theme legcons:Item .

C2020A00012:355 a legcons:Item,
        owl:Class,
        dcat:Resource ;
    rdfs:label "Item - I355 249  Conduct that contravenes rules"@en-AU ;
    dct:isPartOf C2020A00012:351 ;
    dct:isReferencedBy C2020A00012: ;
    rdfs:comment "249  Conduct that contravenes rules - Abrievated Graph Key: I355"@en-AU ;
    skos:definition "249  Conduct that contravenes rules"@en-AU ;
    skos:narrower C2020A00012:351 ;
    skos:prefLabel "Item I355"@en-AU ;
    dcat:accessURL <https://www.legislation.gov.au/C2020A00012/2024-07-10/2024-07-10/text/original/epub/OEBPS/document_1/document_1.html#_Toc172119047> ;
    dcat:landingPage "https://www.legislation.gov.au/C2020A00012/2024-07-10/2024-07-10/text/original/epub/OEBPS/document_1/document_1.html#_Toc172119047"^^xsd:anyURI ;
    dcat:theme legcons:Item .

C2020A00012:356 a legcons:Item,
        owl:Class,
        dcat:Resource ;
    rdfs:label "Item - I356 250  Alteration of or interference with trade description"@en-AU ;
    dct:isPartOf C2020A00012:351 ;
    dct:isReferencedBy C2020A00012: ;
    rdfs:comment "250  Alteration of or interference with trade description - Abrievated Graph Key: I356"@en-AU ;
    skos:definition "250  Alteration of or interference with trade description"@en-AU ;
    skos:narrower C2020A00012:351 ;
    skos:prefLabel "Item I356"@en-AU ;
    dcat:accessURL <https://www.legislation.gov.au/C2020A00012/2024-07-10/2024-07-10/text/original/epub/OEBPS/document_1/document_1.html#_Toc172119048> ;
    dcat:landingPage "https://www.legislation.gov.au/C2020A00012/2024-07-10/2024-07-10/text/original/epub/OEBPS/document_1/document_1.html#_Toc172119048"^^xsd:anyURI ;
    dcat:theme legcons:Item .

C2020A00012:358 a legcons:Item,
        owl:Class,
        dcat:Resource ;
    rdfs:label "Item - I358 251  Meaning of false trade description"@en-AU ;
    dct:isPartOf C2020A00012:357 ;
    dct:isReferencedBy C2020A00012: ;
    rdfs:comment "251  Meaning of false trade description - Abrievated Graph Key: I358"@en-AU ;
    skos:definition "251  Meaning of false trade description"@en-AU ;
    skos:narrower C2020A00012:357 ;
    skos:prefLabel "Item I358"@en-AU ;
    dcat:accessURL <https://www.legislation.gov.au/C2020A00012/2024-07-10/2024-07-10/text/original/epub/OEBPS/document_1/document_1.html#_Toc172119050> ;
    dcat:landingPage "https://www.legislation.gov.au/C2020A00012/2024-07-10/2024-07-10/text/original/epub/OEBPS/document_1/document_1.html#_Toc172119050"^^xsd:anyURI ;
    dcat:theme legcons:Item .

C2020A00012:359 a legcons:Item,
        owl:Class,
        dcat:Resource ;
    rdfs:label "Item - I359 252  False trade description must not be applied to prescribed goods"@en-AU ;
    dct:isPartOf C2020A00012:357 ;
    dct:isReferencedBy C2020A00012: ;
    rdfs:comment "252  False trade description must not be applied to prescribed goods - Abrievated Graph Key: I359"@en-AU ;
    skos:definition "252  False trade description must not be applied to prescribed goods"@en-AU ;
    skos:narrower C2020A00012:357 ;
    skos:prefLabel "Item I359"@en-AU ;
    dcat:accessURL <https://www.legislation.gov.au/C2020A00012/2024-07-10/2024-07-10/text/original/epub/OEBPS/document_1/document_1.html#_Toc172119051> ;
    dcat:landingPage "https://www.legislation.gov.au/C2020A00012/2024-07-10/2024-07-10/text/original/epub/OEBPS/document_1/document_1.html#_Toc172119051"^^xsd:anyURI ;
    dcat:theme legcons:Item .

C2020A00012:36 a legcons:Item,
        owl:Class,
        dcat:Resource ;
    rdfs:label "Item - I36 24  Minister may temporarily prohibit export of goods from Australian territory or from a part of Australian territory for a period"@en-AU ;
    dct:isPartOf C2020A00012:31 ;
    dct:isReferencedBy C2020A00012: ;
    rdfs:comment "24  Minister may temporarily prohibit export of goods from Australian territory or from a part of Australian territory for a period - Abrievated Graph Key: I36"@en-AU ;
    skos:definition "24  Minister may temporarily prohibit export of goods from Australian territory or from a part of Australian territory for a period"@en-AU ;
    skos:narrower C2020A00012:31 ;
    skos:prefLabel "Item I36"@en-AU ;
    dcat:accessURL <https://www.legislation.gov.au/C2020A00012/2024-07-10/2024-07-10/text/original/epub/OEBPS/document_1/document_1.html#_Toc172118728> ;
    dcat:landingPage "https://www.legislation.gov.au/C2020A00012/2024-07-10/2024-07-10/text/original/epub/OEBPS/document_1/document_1.html#_Toc172118728"^^xsd:anyURI ;
    dcat:theme legcons:Item .

C2020A00012:360 a legcons:Item,
        owl:Class,
        dcat:Resource ;
    rdfs:label "Item - I360 253  Goods with false trade description must not be exported etc"@en-AU ;
    dct:isPartOf C2020A00012:357 ;
    dct:isReferencedBy C2020A00012: ;
    rdfs:comment "253  Goods with false trade description must not be exported etc - Abrievated Graph Key: I360"@en-AU ;
    skos:definition "253  Goods with false trade description must not be exported etc"@en-AU ;
    skos:narrower C2020A00012:357 ;
    skos:prefLabel "Item I360"@en-AU ;
    dcat:accessURL <https://www.legislation.gov.au/C2020A00012/2024-07-10/2024-07-10/text/original/epub/OEBPS/document_1/document_1.html#_Toc172119052> ;
    dcat:landingPage "https://www.legislation.gov.au/C2020A00012/2024-07-10/2024-07-10/text/original/epub/OEBPS/document_1/document_1.html#_Toc172119052"^^xsd:anyURI ;
    dcat:theme legcons:Item .

C2020A00012:363 a legcons:Item,
        owl:Class,
        dcat:Resource ;
    rdfs:label "Item - I363 254  Simplified outline of this Part"@en-AU ;
    dct:isPartOf C2020A00012:362 ;
    dct:isReferencedBy C2020A00012: ;
    rdfs:comment "254  Simplified outline of this Part - Abrievated Graph Key: I363"@en-AU ;
    skos:definition "254  Simplified outline of this Part"@en-AU ;
    skos:narrower C2020A00012:362 ;
    skos:prefLabel "Item I363"@en-AU ;
    dcat:accessURL <https://www.legislation.gov.au/C2020A00012/2024-07-10/2024-07-10/text/original/epub/OEBPS/document_1/document_1.html#_Toc172119055> ;
    dcat:landingPage "https://www.legislation.gov.au/C2020A00012/2024-07-10/2024-07-10/text/original/epub/OEBPS/document_1/document_1.html#_Toc172119055"^^xsd:anyURI ;
    dcat:theme legcons:Item .

C2020A00012:365 a legcons:Item,
        owl:Class,
        dcat:Resource ;
    rdfs:label "Item - I365 255  Official marks"@en-AU ;
    dct:isPartOf C2020A00012:364 ;
    dct:isReferencedBy C2020A00012: ;
    rdfs:comment "255  Official marks - Abrievated Graph Key: I365"@en-AU ;
    skos:definition "255  Official marks"@en-AU ;
    skos:narrower C2020A00012:364 ;
    skos:prefLabel "Item I365"@en-AU ;
    dcat:accessURL <https://www.legislation.gov.au/C2020A00012/2024-07-10/2024-07-10/text/original/epub/OEBPS/document_1/document_1.html#_Toc172119057> ;
    dcat:landingPage "https://www.legislation.gov.au/C2020A00012/2024-07-10/2024-07-10/text/original/epub/OEBPS/document_1/document_1.html#_Toc172119057"^^xsd:anyURI ;
    dcat:theme legcons:Item .

C2020A00012:366 a legcons:Item,
        owl:Class,
        dcat:Resource ;
    rdfs:label "Item - I366 256  Marks resembling official marks"@en-AU ;
    dct:isPartOf C2020A00012:364 ;
    dct:isReferencedBy C2020A00012: ;
    rdfs:comment "256  Marks resembling official marks - Abrievated Graph Key: I366"@en-AU ;
    skos:definition "256  Marks resembling official marks"@en-AU ;
    skos:narrower C2020A00012:364 ;
    skos:prefLabel "Item I366"@en-AU ;
    dcat:accessURL <https://www.legislation.gov.au/C2020A00012/2024-07-10/2024-07-10/text/original/epub/OEBPS/document_1/document_1.html#_Toc172119058> ;
    dcat:landingPage "https://www.legislation.gov.au/C2020A00012/2024-07-10/2024-07-10/text/original/epub/OEBPS/document_1/document_1.html#_Toc172119058"^^xsd:anyURI ;
    dcat:theme legcons:Item .

C2020A00012:367 a legcons:Item,
        owl:Class,
        dcat:Resource ;
    rdfs:label "Item - I367 257  Official marking devices"@en-AU ;
    dct:isPartOf C2020A00012:364 ;
    dct:isReferencedBy C2020A00012: ;
    rdfs:comment "257  Official marking devices - Abrievated Graph Key: I367"@en-AU ;
    skos:definition "257  Official marking devices"@en-AU ;
    skos:narrower C2020A00012:364 ;
    skos:prefLabel "Item I367"@en-AU ;
    dcat:accessURL <https://www.legislation.gov.au/C2020A00012/2024-07-10/2024-07-10/text/original/epub/OEBPS/document_1/document_1.html#_Toc172119059> ;
    dcat:landingPage "https://www.legislation.gov.au/C2020A00012/2024-07-10/2024-07-10/text/original/epub/OEBPS/document_1/document_1.html#_Toc172119059"^^xsd:anyURI ;
    dcat:theme legcons:Item .

C2020A00012:369 a legcons:Item,
        owl:Class,
        dcat:Resource ;
    rdfs:label "Item - I369 258  Conduct that contravenes rules"@en-AU ;
    dct:isPartOf C2020A00012:368 ;
    dct:isReferencedBy C2020A00012: ;
    rdfs:comment "258  Conduct that contravenes rules - Abrievated Graph Key: I369"@en-AU ;
    skos:definition "258  Conduct that contravenes rules"@en-AU ;
    skos:narrower C2020A00012:368 ;
    skos:prefLabel "Item I369"@en-AU ;
    dcat:accessURL <https://www.legislation.gov.au/C2020A00012/2024-07-10/2024-07-10/text/original/epub/OEBPS/document_1/document_1.html#_Toc172119061> ;
    dcat:landingPage "https://www.legislation.gov.au/C2020A00012/2024-07-10/2024-07-10/text/original/epub/OEBPS/document_1/document_1.html#_Toc172119061"^^xsd:anyURI ;
    dcat:theme legcons:Item .

C2020A00012:37 a legcons:Item,
        owl:Class,
        dcat:Resource ;
    rdfs:label "Item - I37 25  Variation of temporary prohibition determination"@en-AU ;
    dct:isPartOf C2020A00012:31 ;
    dct:isReferencedBy C2020A00012: ;
    rdfs:comment "25  Variation of temporary prohibition determination - Abrievated Graph Key: I37"@en-AU ;
    skos:definition "25  Variation of temporary prohibition determination"@en-AU ;
    skos:narrower C2020A00012:31 ;
    skos:prefLabel "Item I37"@en-AU ;
    dcat:accessURL <https://www.legislation.gov.au/C2020A00012/2024-07-10/2024-07-10/text/original/epub/OEBPS/document_1/document_1.html#_Toc172118729> ;
    dcat:landingPage "https://www.legislation.gov.au/C2020A00012/2024-07-10/2024-07-10/text/original/epub/OEBPS/document_1/document_1.html#_Toc172118729"^^xsd:anyURI ;
    dcat:theme legcons:Item .

C2020A00012:370 a legcons:Item,
        owl:Class,
        dcat:Resource ;
    rdfs:label "Item - I370 259  Applying a false misleading or deceptive official mark to goods"@en-AU ;
    dct:isPartOf C2020A00012:368 ;
    dct:isReferencedBy C2020A00012: ;
    rdfs:comment "259  Applying a false misleading or deceptive official mark to goods - Abrievated Graph Key: I370"@en-AU ;
    skos:definition "259  Applying a false misleading or deceptive official mark to goods"@en-AU ;
    skos:narrower C2020A00012:368 ;
    skos:prefLabel "Item I370"@en-AU ;
    dcat:accessURL <https://www.legislation.gov.au/C2020A00012/2024-07-10/2024-07-10/text/original/epub/OEBPS/document_1/document_1.html#_Toc172119062> ;
    dcat:landingPage "https://www.legislation.gov.au/C2020A00012/2024-07-10/2024-07-10/text/original/epub/OEBPS/document_1/document_1.html#_Toc172119062"^^xsd:anyURI ;
    dcat:theme legcons:Item .

C2020A00012:371 a legcons:Item,
        owl:Class,
        dcat:Resource ;
    rdfs:label "Item - I371 260  Applying a false misleading or deceptive official mark to a document"@en-AU ;
    dct:isPartOf C2020A00012:368 ;
    dct:isReferencedBy C2020A00012: ;
    rdfs:comment "260  Applying a false misleading or deceptive official mark to a document - Abrievated Graph Key: I371"@en-AU ;
    skos:definition "260  Applying a false misleading or deceptive official mark to a document"@en-AU ;
    skos:narrower C2020A00012:368 ;
    skos:prefLabel "Item I371"@en-AU ;
    dcat:accessURL <https://www.legislation.gov.au/C2020A00012/2024-07-10/2024-07-10/text/original/epub/OEBPS/document_1/document_1.html#_Toc172119063> ;
    dcat:landingPage "https://www.legislation.gov.au/C2020A00012/2024-07-10/2024-07-10/text/original/epub/OEBPS/document_1/document_1.html#_Toc172119063"^^xsd:anyURI ;
    dcat:theme legcons:Item .

C2020A00012:372 a legcons:Item,
        owl:Class,
        dcat:Resource ;
    rdfs:label "Item - I372 261  Conduct that results in official mark applied to goods being altered to be false misleading or deceptive"@en-AU ;
    dct:isPartOf C2020A00012:368 ;
    dct:isReferencedBy C2020A00012: ;
    rdfs:comment "261  Conduct that results in official mark applied to goods being altered to be false misleading or deceptive - Abrievated Graph Key: I372"@en-AU ;
    skos:definition "261  Conduct that results in official mark applied to goods being altered to be false misleading or deceptive"@en-AU ;
    skos:narrower C2020A00012:368 ;
    skos:prefLabel "Item I372"@en-AU ;
    dcat:accessURL <https://www.legislation.gov.au/C2020A00012/2024-07-10/2024-07-10/text/original/epub/OEBPS/document_1/document_1.html#_Toc172119064> ;
    dcat:landingPage "https://www.legislation.gov.au/C2020A00012/2024-07-10/2024-07-10/text/original/epub/OEBPS/document_1/document_1.html#_Toc172119064"^^xsd:anyURI ;
    dcat:theme legcons:Item .

C2020A00012:373 a legcons:Item,
        owl:Class,
        dcat:Resource ;
    rdfs:label "Item - I373 262  Conduct that results in official mark applied to a document being altered to be false misleading or deceptive"@en-AU ;
    dct:isPartOf C2020A00012:368 ;
    dct:isReferencedBy C2020A00012: ;
    rdfs:comment "262  Conduct that results in official mark applied to a document being altered to be false misleading or deceptive - Abrievated Graph Key: I373"@en-AU ;
    skos:definition "262  Conduct that results in official mark applied to a document being altered to be false misleading or deceptive"@en-AU ;
    skos:narrower C2020A00012:368 ;
    skos:prefLabel "Item I373"@en-AU ;
    dcat:accessURL <https://www.legislation.gov.au/C2020A00012/2024-07-10/2024-07-10/text/original/epub/OEBPS/document_1/document_1.html#_Toc172119065> ;
    dcat:landingPage "https://www.legislation.gov.au/C2020A00012/2024-07-10/2024-07-10/text/original/epub/OEBPS/document_1/document_1.html#_Toc172119065"^^xsd:anyURI ;
    dcat:theme legcons:Item .

C2020A00012:376 a legcons:Item,
        owl:Class,
        dcat:Resource ;
    rdfs:label "Item - I376 263  Simplified outline of this Part"@en-AU ;
    dct:isPartOf C2020A00012:375 ;
    dct:isReferencedBy C2020A00012: ;
    rdfs:comment "263  Simplified outline of this Part - Abrievated Graph Key: I376"@en-AU ;
    skos:definition "263  Simplified outline of this Part"@en-AU ;
    skos:narrower C2020A00012:375 ;
    skos:prefLabel "Item I376"@en-AU ;
    dcat:accessURL <https://www.legislation.gov.au/C2020A00012/2024-07-10/2024-07-10/text/original/epub/OEBPS/document_1/document_1.html#_Toc172119068> ;
    dcat:landingPage "https://www.legislation.gov.au/C2020A00012/2024-07-10/2024-07-10/text/original/epub/OEBPS/document_1/document_1.html#_Toc172119068"^^xsd:anyURI ;
    dcat:theme legcons:Item .

C2020A00012:378 a legcons:Item,
        owl:Class,
        dcat:Resource ;
    rdfs:label "Item - I378 264  Tariff rate quota systems"@en-AU ;
    dct:isPartOf C2020A00012:377 ;
    dct:isReferencedBy C2020A00012: ;
    rdfs:comment "264  Tariff rate quota systems - Abrievated Graph Key: I378"@en-AU ;
    skos:definition "264  Tariff rate quota systems"@en-AU ;
    skos:narrower C2020A00012:377 ;
    skos:prefLabel "Item I378"@en-AU ;
    dcat:accessURL <https://www.legislation.gov.au/C2020A00012/2024-07-10/2024-07-10/text/original/epub/OEBPS/document_1/document_1.html#_Toc172119070> ;
    dcat:landingPage "https://www.legislation.gov.au/C2020A00012/2024-07-10/2024-07-10/text/original/epub/OEBPS/document_1/document_1.html#_Toc172119070"^^xsd:anyURI ;
    dcat:theme legcons:Item .

C2020A00012:38 a legcons:Item,
        owl:Class,
        dcat:Resource ;
    rdfs:label "Item - I38 26  Effect of temporary prohibition determination on government certificate or export permit"@en-AU ;
    dct:isPartOf C2020A00012:31 ;
    dct:isReferencedBy C2020A00012: ;
    rdfs:comment "26  Effect of temporary prohibition determination on government certificate or export permit - Abrievated Graph Key: I38"@en-AU ;
    skos:definition "26  Effect of temporary prohibition determination on government certificate or export permit"@en-AU ;
    skos:narrower C2020A00012:31 ;
    skos:prefLabel "Item I38"@en-AU ;
    dcat:accessURL <https://www.legislation.gov.au/C2020A00012/2024-07-10/2024-07-10/text/original/epub/OEBPS/document_1/document_1.html#_Toc172118730> ;
    dcat:landingPage "https://www.legislation.gov.au/C2020A00012/2024-07-10/2024-07-10/text/original/epub/OEBPS/document_1/document_1.html#_Toc172118730"^^xsd:anyURI ;
    dcat:theme legcons:Item .

C2020A00012:382 a legcons:Item,
        owl:Class,
        dcat:Resource ;
    rdfs:label "Item - I382 265  Simplified outline of this Part"@en-AU ;
    dct:isPartOf C2020A00012:381 ;
    dct:isReferencedBy C2020A00012: ;
    rdfs:comment "265  Simplified outline of this Part - Abrievated Graph Key: I382"@en-AU ;
    skos:definition "265  Simplified outline of this Part"@en-AU ;
    skos:narrower C2020A00012:381 ;
    skos:prefLabel "Item I382"@en-AU ;
    dcat:accessURL <https://www.legislation.gov.au/C2020A00012/2024-07-10/2024-07-10/text/original/epub/OEBPS/document_1/document_1.html#_Toc172119074> ;
    dcat:landingPage "https://www.legislation.gov.au/C2020A00012/2024-07-10/2024-07-10/text/original/epub/OEBPS/document_1/document_1.html#_Toc172119074"^^xsd:anyURI ;
    dcat:theme legcons:Item .

C2020A00012:384 a legcons:Item,
        owl:Class,
        dcat:Resource ;
    rdfs:label "Item - I384 266  Audits of export operations"@en-AU ;
    dct:isPartOf C2020A00012:383 ;
    dct:isReferencedBy C2020A00012: ;
    rdfs:comment "266  Audits of export operations - Abrievated Graph Key: I384"@en-AU ;
    skos:definition "266  Audits of export operations"@en-AU ;
    skos:narrower C2020A00012:383 ;
    skos:prefLabel "Item I384"@en-AU ;
    dcat:accessURL <https://www.legislation.gov.au/C2020A00012/2024-07-10/2024-07-10/text/original/epub/OEBPS/document_1/document_1.html#_Toc172119076> ;
    dcat:landingPage "https://www.legislation.gov.au/C2020A00012/2024-07-10/2024-07-10/text/original/epub/OEBPS/document_1/document_1.html#_Toc172119076"^^xsd:anyURI ;
    dcat:theme legcons:Item .

C2020A00012:385 a legcons:Item,
        owl:Class,
        dcat:Resource ;
    rdfs:label "Item - I385 267  Audits in relation to persons performing functions or exercising powers under this Act"@en-AU ;
    dct:isPartOf C2020A00012:383 ;
    dct:isReferencedBy C2020A00012: ;
    rdfs:comment "267  Audits in relation to persons performing functions or exercising powers under this Act - Abrievated Graph Key: I385"@en-AU ;
    skos:definition "267  Audits in relation to persons performing functions or exercising powers under this Act"@en-AU ;
    skos:narrower C2020A00012:383 ;
    skos:prefLabel "Item I385"@en-AU ;
    dcat:accessURL <https://www.legislation.gov.au/C2020A00012/2024-07-10/2024-07-10/text/original/epub/OEBPS/document_1/document_1.html#_Toc172119077> ;
    dcat:landingPage "https://www.legislation.gov.au/C2020A00012/2024-07-10/2024-07-10/text/original/epub/OEBPS/document_1/document_1.html#_Toc172119077"^^xsd:anyURI ;
    dcat:theme legcons:Item .

C2020A00012:386 a legcons:Item,
        owl:Class,
        dcat:Resource ;
    rdfs:label "Item - I386 268  Single audit or program of audits may be required"@en-AU ;
    dct:isPartOf C2020A00012:383 ;
    dct:isReferencedBy C2020A00012: ;
    rdfs:comment "268  Single audit or program of audits may be required - Abrievated Graph Key: I386"@en-AU ;
    skos:definition "268  Single audit or program of audits may be required"@en-AU ;
    skos:narrower C2020A00012:383 ;
    skos:prefLabel "Item I386"@en-AU ;
    dcat:accessURL <https://www.legislation.gov.au/C2020A00012/2024-07-10/2024-07-10/text/original/epub/OEBPS/document_1/document_1.html#_Toc172119078> ;
    dcat:landingPage "https://www.legislation.gov.au/C2020A00012/2024-07-10/2024-07-10/text/original/epub/OEBPS/document_1/document_1.html#_Toc172119078"^^xsd:anyURI ;
    dcat:theme legcons:Item .

C2020A00012:387 a legcons:Item,
        owl:Class,
        dcat:Resource ;
    rdfs:label "Item - I387 269  Relevant person for an audit"@en-AU ;
    dct:isPartOf C2020A00012:383 ;
    dct:isReferencedBy C2020A00012: ;
    rdfs:comment "269  Relevant person for an audit - Abrievated Graph Key: I387"@en-AU ;
    skos:definition "269  Relevant person for an audit"@en-AU ;
    skos:narrower C2020A00012:383 ;
    skos:prefLabel "Item I387"@en-AU ;
    dcat:accessURL <https://www.legislation.gov.au/C2020A00012/2024-07-10/2024-07-10/text/original/epub/OEBPS/document_1/document_1.html#_Toc172119079> ;
    dcat:landingPage "https://www.legislation.gov.au/C2020A00012/2024-07-10/2024-07-10/text/original/epub/OEBPS/document_1/document_1.html#_Toc172119079"^^xsd:anyURI ;
    dcat:theme legcons:Item .

C2020A00012:388 a legcons:Item,
        owl:Class,
        dcat:Resource ;
    rdfs:label "Item - I388 270  Conduct of audit"@en-AU ;
    dct:isPartOf C2020A00012:383 ;
    dct:isReferencedBy C2020A00012: ;
    rdfs:comment "270  Conduct of audit - Abrievated Graph Key: I388"@en-AU ;
    skos:definition "270  Conduct of audit"@en-AU ;
    skos:narrower C2020A00012:383 ;
    skos:prefLabel "Item I388"@en-AU ;
    dcat:accessURL <https://www.legislation.gov.au/C2020A00012/2024-07-10/2024-07-10/text/original/epub/OEBPS/document_1/document_1.html#_Toc172119080> ;
    dcat:landingPage "https://www.legislation.gov.au/C2020A00012/2024-07-10/2024-07-10/text/original/epub/OEBPS/document_1/document_1.html#_Toc172119080"^^xsd:anyURI ;
    dcat:theme legcons:Item .

C2020A00012:389 a legcons:Item,
        owl:Class,
        dcat:Resource ;
    rdfs:label "Item - I389 271  Relevant person for an audit must provide assistance"@en-AU ;
    dct:isPartOf C2020A00012:383 ;
    dct:isReferencedBy C2020A00012: ;
    rdfs:comment "271  Relevant person for an audit must provide assistance - Abrievated Graph Key: I389"@en-AU ;
    skos:definition "271  Relevant person for an audit must provide assistance"@en-AU ;
    skos:narrower C2020A00012:383 ;
    skos:prefLabel "Item I389"@en-AU ;
    dcat:accessURL <https://www.legislation.gov.au/C2020A00012/2024-07-10/2024-07-10/text/original/epub/OEBPS/document_1/document_1.html#_Toc172119081> ;
    dcat:landingPage "https://www.legislation.gov.au/C2020A00012/2024-07-10/2024-07-10/text/original/epub/OEBPS/document_1/document_1.html#_Toc172119081"^^xsd:anyURI ;
    dcat:theme legcons:Item .

C2020A00012:39 a legcons:Item,
        owl:Class,
        dcat:Resource ;
    rdfs:label "Item - I39 27  Temporary prohibition determination prevails over inconsistent rules"@en-AU ;
    dct:isPartOf C2020A00012:31 ;
    dct:isReferencedBy C2020A00012: ;
    rdfs:comment "27  Temporary prohibition determination prevails over inconsistent rules - Abrievated Graph Key: I39"@en-AU ;
    skos:definition "27  Temporary prohibition determination prevails over inconsistent rules"@en-AU ;
    skos:narrower C2020A00012:31 ;
    skos:prefLabel "Item I39"@en-AU ;
    dcat:accessURL <https://www.legislation.gov.au/C2020A00012/2024-07-10/2024-07-10/text/original/epub/OEBPS/document_1/document_1.html#_Toc172118731> ;
    dcat:landingPage "https://www.legislation.gov.au/C2020A00012/2024-07-10/2024-07-10/text/original/epub/OEBPS/document_1/document_1.html#_Toc172118731"^^xsd:anyURI ;
    dcat:theme legcons:Item .

C2020A00012:390 a legcons:Item,
        owl:Class,
        dcat:Resource ;
    rdfs:label "Item - I390 272  Powers of auditors"@en-AU ;
    dct:isPartOf C2020A00012:383 ;
    dct:isReferencedBy C2020A00012: ;
    rdfs:comment "272  Powers of auditors - Abrievated Graph Key: I390"@en-AU ;
    skos:definition "272  Powers of auditors"@en-AU ;
    skos:narrower C2020A00012:383 ;
    skos:prefLabel "Item I390"@en-AU ;
    dcat:accessURL <https://www.legislation.gov.au/C2020A00012/2024-07-10/2024-07-10/text/original/epub/OEBPS/document_1/document_1.html#_Toc172119082> ;
    dcat:landingPage "https://www.legislation.gov.au/C2020A00012/2024-07-10/2024-07-10/text/original/epub/OEBPS/document_1/document_1.html#_Toc172119082"^^xsd:anyURI ;
    dcat:theme legcons:Item .

C2020A00012:392 a legcons:Item,
        owl:Class,
        dcat:Resource ;
    rdfs:label "Item - I392 273  Secretary may approve persons to conduct audits"@en-AU ;
    dct:isPartOf C2020A00012:391 ;
    dct:isReferencedBy C2020A00012: ;
    rdfs:comment "273  Secretary may approve persons to conduct audits - Abrievated Graph Key: I392"@en-AU ;
    skos:definition "273  Secretary may approve persons to conduct audits"@en-AU ;
    skos:narrower C2020A00012:391 ;
    skos:prefLabel "Item I392"@en-AU ;
    dcat:accessURL <https://www.legislation.gov.au/C2020A00012/2024-07-10/2024-07-10/text/original/epub/OEBPS/document_1/document_1.html#_Toc172119084> ;
    dcat:landingPage "https://www.legislation.gov.au/C2020A00012/2024-07-10/2024-07-10/text/original/epub/OEBPS/document_1/document_1.html#_Toc172119084"^^xsd:anyURI ;
    dcat:theme legcons:Item .

C2020A00012:393 a legcons:Item,
        owl:Class,
        dcat:Resource ;
    rdfs:label "Item - I393 274  Rules may provide for classes of persons to be auditors"@en-AU ;
    dct:isPartOf C2020A00012:391 ;
    dct:isReferencedBy C2020A00012: ;
    rdfs:comment "274  Rules may provide for classes of persons to be auditors - Abrievated Graph Key: I393"@en-AU ;
    skos:definition "274  Rules may provide for classes of persons to be auditors"@en-AU ;
    skos:narrower C2020A00012:391 ;
    skos:prefLabel "Item I393"@en-AU ;
    dcat:accessURL <https://www.legislation.gov.au/C2020A00012/2024-07-10/2024-07-10/text/original/epub/OEBPS/document_1/document_1.html#_Toc172119085> ;
    dcat:landingPage "https://www.legislation.gov.au/C2020A00012/2024-07-10/2024-07-10/text/original/epub/OEBPS/document_1/document_1.html#_Toc172119085"^^xsd:anyURI ;
    dcat:theme legcons:Item .

C2020A00012:394 a legcons:Item,
        owl:Class,
        dcat:Resource ;
    rdfs:label "Item - I394 275  Approved auditors may charge fees"@en-AU ;
    dct:isPartOf C2020A00012:391 ;
    dct:isReferencedBy C2020A00012: ;
    rdfs:comment "275  Approved auditors may charge fees - Abrievated Graph Key: I394"@en-AU ;
    skos:definition "275  Approved auditors may charge fees"@en-AU ;
    skos:narrower C2020A00012:391 ;
    skos:prefLabel "Item I394"@en-AU ;
    dcat:accessURL <https://www.legislation.gov.au/C2020A00012/2024-07-10/2024-07-10/text/original/epub/OEBPS/document_1/document_1.html#_Toc172119086> ;
    dcat:landingPage "https://www.legislation.gov.au/C2020A00012/2024-07-10/2024-07-10/text/original/epub/OEBPS/document_1/document_1.html#_Toc172119086"^^xsd:anyURI ;
    dcat:theme legcons:Item .

C2020A00012:397 a legcons:Item,
        owl:Class,
        dcat:Resource ;
    rdfs:label "Item - I397 276  Simplified outline of this Part"@en-AU ;
    dct:isPartOf C2020A00012:396 ;
    dct:isReferencedBy C2020A00012: ;
    rdfs:comment "276  Simplified outline of this Part - Abrievated Graph Key: I397"@en-AU ;
    skos:definition "276  Simplified outline of this Part"@en-AU ;
    skos:narrower C2020A00012:396 ;
    skos:prefLabel "Item I397"@en-AU ;
    dcat:accessURL <https://www.legislation.gov.au/C2020A00012/2024-07-10/2024-07-10/text/original/epub/OEBPS/document_1/document_1.html#_Toc172119089> ;
    dcat:landingPage "https://www.legislation.gov.au/C2020A00012/2024-07-10/2024-07-10/text/original/epub/OEBPS/document_1/document_1.html#_Toc172119089"^^xsd:anyURI ;
    dcat:theme legcons:Item .

C2020A00012:399 a legcons:Item,
        owl:Class,
        dcat:Resource ;
    rdfs:label "Item - I399 277  Circumstances in which an assessment may be carried out etc"@en-AU ;
    dct:isPartOf C2020A00012:398 ;
    dct:isReferencedBy C2020A00012: ;
    rdfs:comment "277  Circumstances in which an assessment may be carried out etc - Abrievated Graph Key: I399"@en-AU ;
    skos:definition "277  Circumstances in which an assessment may be carried out etc"@en-AU ;
    skos:narrower C2020A00012:398 ;
    skos:prefLabel "Item I399"@en-AU ;
    dcat:accessURL <https://www.legislation.gov.au/C2020A00012/2024-07-10/2024-07-10/text/original/epub/OEBPS/document_1/document_1.html#_Toc172119091> ;
    dcat:landingPage "https://www.legislation.gov.au/C2020A00012/2024-07-10/2024-07-10/text/original/epub/OEBPS/document_1/document_1.html#_Toc172119091"^^xsd:anyURI ;
    dcat:theme legcons:Item .

C2020A00012:4 a legcons:Item,
        owl:Class,
        dcat:Resource ;
    rdfs:label "Item - I4 2  Commencement"@en-AU ;
    dct:isPartOf C2020A00012:1 ;
    dct:isReferencedBy C2020A00012: ;
    rdfs:comment "2  Commencement - Abrievated Graph Key: I4"@en-AU ;
    skos:definition "2  Commencement"@en-AU ;
    skos:narrower C2020A00012:1 ;
    skos:prefLabel "Item I4"@en-AU ;
    dcat:accessURL <https://www.legislation.gov.au/C2020A00012/2024-07-10/2024-07-10/text/original/epub/OEBPS/document_1/document_1.html#_Toc172118696> ;
    dcat:landingPage "https://www.legislation.gov.au/C2020A00012/2024-07-10/2024-07-10/text/original/epub/OEBPS/document_1/document_1.html#_Toc172118696"^^xsd:anyURI ;
    dcat:theme legcons:Item .

C2020A00012:40 a legcons:Division,
        owl:Class,
        dcat:Resource ;
    rdfs:label "Division - D40 Division 3 Prescribed goods and conditions of export"@en-AU ;
    dct:isPartOf C2020A00012:28 ;
    dct:isReferencedBy C2020A00012: ;
    rdfs:comment "Division 3 Prescribed goods and conditions of export - Abrievated Graph Key: D40"@en-AU ;
    skos:definition "Division 3 Prescribed goods and conditions of export"@en-AU ;
    skos:narrower C2020A00012:28 ;
    skos:prefLabel "Division D40"@en-AU ;
    dcat:accessURL <https://www.legislation.gov.au/C2020A00012/2024-07-10/2024-07-10/text/original/epub/OEBPS/document_1/document_1.html#_Toc172118732> ;
    dcat:landingPage "https://www.legislation.gov.au/C2020A00012/2024-07-10/2024-07-10/text/original/epub/OEBPS/document_1/document_1.html#_Toc172118732"^^xsd:anyURI ;
    dcat:theme legcons:Division .

C2020A00012:400 a legcons:Item,
        owl:Class,
        dcat:Resource ;
    rdfs:label "Item - I400 278  Relevant person for an assessment of goods"@en-AU ;
    dct:isPartOf C2020A00012:398 ;
    dct:isReferencedBy C2020A00012: ;
    rdfs:comment "278  Relevant person for an assessment of goods - Abrievated Graph Key: I400"@en-AU ;
    skos:definition "278  Relevant person for an assessment of goods"@en-AU ;
    skos:narrower C2020A00012:398 ;
    skos:prefLabel "Item I400"@en-AU ;
    dcat:accessURL <https://www.legislation.gov.au/C2020A00012/2024-07-10/2024-07-10/text/original/epub/OEBPS/document_1/document_1.html#_Toc172119092> ;
    dcat:landingPage "https://www.legislation.gov.au/C2020A00012/2024-07-10/2024-07-10/text/original/epub/OEBPS/document_1/document_1.html#_Toc172119092"^^xsd:anyURI ;
    dcat:theme legcons:Item .

C2020A00012:401 a legcons:Item,
        owl:Class,
        dcat:Resource ;
    rdfs:label "Item - I401 279  Process for carrying out an assessment of goods etc"@en-AU ;
    dct:isPartOf C2020A00012:398 ;
    dct:isReferencedBy C2020A00012: ;
    rdfs:comment "279  Process for carrying out an assessment of goods etc - Abrievated Graph Key: I401"@en-AU ;
    skos:definition "279  Process for carrying out an assessment of goods etc"@en-AU ;
    skos:narrower C2020A00012:398 ;
    skos:prefLabel "Item I401"@en-AU ;
    dcat:accessURL <https://www.legislation.gov.au/C2020A00012/2024-07-10/2024-07-10/text/original/epub/OEBPS/document_1/document_1.html#_Toc172119093> ;
    dcat:landingPage "https://www.legislation.gov.au/C2020A00012/2024-07-10/2024-07-10/text/original/epub/OEBPS/document_1/document_1.html#_Toc172119093"^^xsd:anyURI ;
    dcat:theme legcons:Item .

C2020A00012:402 a legcons:Item,
        owl:Class,
        dcat:Resource ;
    rdfs:label "Item - I402 280  Powers that may be exercised in carrying out an assessment of goods"@en-AU ;
    dct:isPartOf C2020A00012:398 ;
    dct:isReferencedBy C2020A00012: ;
    rdfs:comment "280  Powers that may be exercised in carrying out an assessment of goods - Abrievated Graph Key: I402"@en-AU ;
    skos:definition "280  Powers that may be exercised in carrying out an assessment of goods"@en-AU ;
    skos:narrower C2020A00012:398 ;
    skos:prefLabel "Item I402"@en-AU ;
    dcat:accessURL <https://www.legislation.gov.au/C2020A00012/2024-07-10/2024-07-10/text/original/epub/OEBPS/document_1/document_1.html#_Toc172119094> ;
    dcat:landingPage "https://www.legislation.gov.au/C2020A00012/2024-07-10/2024-07-10/text/original/epub/OEBPS/document_1/document_1.html#_Toc172119094"^^xsd:anyURI ;
    dcat:theme legcons:Item .

C2020A00012:404 a legcons:Item,
        owl:Class,
        dcat:Resource ;
    rdfs:label "Item - I404 281  Secretary may approve persons to carry out assessments of goods"@en-AU ;
    dct:isPartOf C2020A00012:403 ;
    dct:isReferencedBy C2020A00012: ;
    rdfs:comment "281  Secretary may approve persons to carry out assessments of goods - Abrievated Graph Key: I404"@en-AU ;
    skos:definition "281  Secretary may approve persons to carry out assessments of goods"@en-AU ;
    skos:narrower C2020A00012:403 ;
    skos:prefLabel "Item I404"@en-AU ;
    dcat:accessURL <https://www.legislation.gov.au/C2020A00012/2024-07-10/2024-07-10/text/original/epub/OEBPS/document_1/document_1.html#_Toc172119096> ;
    dcat:landingPage "https://www.legislation.gov.au/C2020A00012/2024-07-10/2024-07-10/text/original/epub/OEBPS/document_1/document_1.html#_Toc172119096"^^xsd:anyURI ;
    dcat:theme legcons:Item .

C2020A00012:405 a legcons:Item,
        owl:Class,
        dcat:Resource ;
    rdfs:label "Item - I405 282  Rules may provide for classes of persons to be assessors"@en-AU ;
    dct:isPartOf C2020A00012:403 ;
    dct:isReferencedBy C2020A00012: ;
    rdfs:comment "282  Rules may provide for classes of persons to be assessors - Abrievated Graph Key: I405"@en-AU ;
    skos:definition "282  Rules may provide for classes of persons to be assessors"@en-AU ;
    skos:narrower C2020A00012:403 ;
    skos:prefLabel "Item I405"@en-AU ;
    dcat:accessURL <https://www.legislation.gov.au/C2020A00012/2024-07-10/2024-07-10/text/original/epub/OEBPS/document_1/document_1.html#_Toc172119097> ;
    dcat:landingPage "https://www.legislation.gov.au/C2020A00012/2024-07-10/2024-07-10/text/original/epub/OEBPS/document_1/document_1.html#_Toc172119097"^^xsd:anyURI ;
    dcat:theme legcons:Item .

C2020A00012:406 a legcons:Item,
        owl:Class,
        dcat:Resource ;
    rdfs:label "Item - I406 283  Approved assessors may charge fees"@en-AU ;
    dct:isPartOf C2020A00012:403 ;
    dct:isReferencedBy C2020A00012: ;
    rdfs:comment "283  Approved assessors may charge fees - Abrievated Graph Key: I406"@en-AU ;
    skos:definition "283  Approved assessors may charge fees"@en-AU ;
    skos:narrower C2020A00012:403 ;
    skos:prefLabel "Item I406"@en-AU ;
    dcat:accessURL <https://www.legislation.gov.au/C2020A00012/2024-07-10/2024-07-10/text/original/epub/OEBPS/document_1/document_1.html#_Toc172119098> ;
    dcat:landingPage "https://www.legislation.gov.au/C2020A00012/2024-07-10/2024-07-10/text/original/epub/OEBPS/document_1/document_1.html#_Toc172119098"^^xsd:anyURI ;
    dcat:theme legcons:Item .

C2020A00012:409 a legcons:Item,
        owl:Class,
        dcat:Resource ;
    rdfs:label "Item - I409 284  Simplified outline of this Part"@en-AU ;
    dct:isPartOf C2020A00012:408 ;
    dct:isReferencedBy C2020A00012: ;
    rdfs:comment "284  Simplified outline of this Part - Abrievated Graph Key: I409"@en-AU ;
    skos:definition "284  Simplified outline of this Part"@en-AU ;
    skos:narrower C2020A00012:408 ;
    skos:prefLabel "Item I409"@en-AU ;
    dcat:accessURL <https://www.legislation.gov.au/C2020A00012/2024-07-10/2024-07-10/text/original/epub/OEBPS/document_1/document_1.html#_Toc172119101> ;
    dcat:landingPage "https://www.legislation.gov.au/C2020A00012/2024-07-10/2024-07-10/text/original/epub/OEBPS/document_1/document_1.html#_Toc172119101"^^xsd:anyURI ;
    dcat:theme legcons:Item .

C2020A00012:41 a legcons:Item,
        owl:Class,
        dcat:Resource ;
    rdfs:label "Item - I41 28  Rules may prescribe goods for the purposes of this Act"@en-AU ;
    dct:isPartOf C2020A00012:28 ;
    dct:isReferencedBy C2020A00012: ;
    rdfs:comment "28  Rules may prescribe goods for the purposes of this Act - Abrievated Graph Key: I41"@en-AU ;
    skos:definition "28  Rules may prescribe goods for the purposes of this Act"@en-AU ;
    skos:narrower C2020A00012:28 ;
    skos:prefLabel "Item I41"@en-AU ;
    dcat:accessURL <https://www.legislation.gov.au/C2020A00012/2024-07-10/2024-07-10/text/original/epub/OEBPS/document_1/document_1.html#_Toc172118733> ;
    dcat:landingPage "https://www.legislation.gov.au/C2020A00012/2024-07-10/2024-07-10/text/original/epub/OEBPS/document_1/document_1.html#_Toc172118733"^^xsd:anyURI ;
    dcat:theme legcons:Item .

C2020A00012:411 a legcons:Item,
        owl:Class,
        dcat:Resource ;
    rdfs:label "Item - I411 285  Power to require information or documents"@en-AU ;
    dct:isPartOf C2020A00012:410 ;
    dct:isReferencedBy C2020A00012: ;
    rdfs:comment "285  Power to require information or documents - Abrievated Graph Key: I411"@en-AU ;
    skos:definition "285  Power to require information or documents"@en-AU ;
    skos:narrower C2020A00012:410 ;
    skos:prefLabel "Item I411"@en-AU ;
    dcat:accessURL <https://www.legislation.gov.au/C2020A00012/2024-07-10/2024-07-10/text/original/epub/OEBPS/document_1/document_1.html#_Toc172119103> ;
    dcat:landingPage "https://www.legislation.gov.au/C2020A00012/2024-07-10/2024-07-10/text/original/epub/OEBPS/document_1/document_1.html#_Toc172119103"^^xsd:anyURI ;
    dcat:theme legcons:Item .

C2020A00012:412 a legcons:Item,
        owl:Class,
        dcat:Resource ;
    rdfs:label "Item - I412 286  Power to arrange for certain decisions to be made by computer programs"@en-AU ;
    dct:isPartOf C2020A00012:410 ;
    dct:isReferencedBy C2020A00012: ;
    rdfs:comment "286  Power to arrange for certain decisions to be made by computer programs - Abrievated Graph Key: I412"@en-AU ;
    skos:definition "286  Power to arrange for certain decisions to be made by computer programs"@en-AU ;
    skos:narrower C2020A00012:410 ;
    skos:prefLabel "Item I412"@en-AU ;
    dcat:accessURL <https://www.legislation.gov.au/C2020A00012/2024-07-10/2024-07-10/text/original/epub/OEBPS/document_1/document_1.html#_Toc172119104> ;
    dcat:landingPage "https://www.legislation.gov.au/C2020A00012/2024-07-10/2024-07-10/text/original/epub/OEBPS/document_1/document_1.html#_Toc172119104"^^xsd:anyURI ;
    dcat:theme legcons:Item .

C2020A00012:413 a legcons:Item,
        owl:Class,
        dcat:Resource ;
    rdfs:label "Item - I413 287  Rules may authorise Commonwealth to enter into arrangements under which money may be paid for certain purposes"@en-AU ;
    dct:isPartOf C2020A00012:410 ;
    dct:isReferencedBy C2020A00012: ;
    rdfs:comment "287  Rules may authorise Commonwealth to enter into arrangements under which money may be paid for certain purposes - Abrievated Graph Key: I413"@en-AU ;
    skos:definition "287  Rules may authorise Commonwealth to enter into arrangements under which money may be paid for certain purposes"@en-AU ;
    skos:narrower C2020A00012:410 ;
    skos:prefLabel "Item I413"@en-AU ;
    dcat:accessURL <https://www.legislation.gov.au/C2020A00012/2024-07-10/2024-07-10/text/original/epub/OEBPS/document_1/document_1.html#_Toc172119105> ;
    dcat:landingPage "https://www.legislation.gov.au/C2020A00012/2024-07-10/2024-07-10/text/original/epub/OEBPS/document_1/document_1.html#_Toc172119105"^^xsd:anyURI ;
    dcat:theme legcons:Item .

C2020A00012:414 a legcons:Item,
        owl:Class,
        dcat:Resource ;
    rdfs:label "Item - I414 288  Delegation and subdelegation"@en-AU ;
    dct:isPartOf C2020A00012:410 ;
    dct:isReferencedBy C2020A00012: ;
    rdfs:comment "288  Delegation and subdelegation - Abrievated Graph Key: I414"@en-AU ;
    skos:definition "288  Delegation and subdelegation"@en-AU ;
    skos:narrower C2020A00012:410 ;
    skos:prefLabel "Item I414"@en-AU ;
    dcat:accessURL <https://www.legislation.gov.au/C2020A00012/2024-07-10/2024-07-10/text/original/epub/OEBPS/document_1/document_1.html#_Toc172119106> ;
    dcat:landingPage "https://www.legislation.gov.au/C2020A00012/2024-07-10/2024-07-10/text/original/epub/OEBPS/document_1/document_1.html#_Toc172119106"^^xsd:anyURI ;
    dcat:theme legcons:Item .

C2020A00012:415 a legcons:Item,
        owl:Class,
        dcat:Resource ;
    rdfs:label "Item - I415 289  Minister may give directions to Secretary"@en-AU ;
    dct:isPartOf C2020A00012:410 ;
    dct:isReferencedBy C2020A00012: ;
    rdfs:comment "289  Minister may give directions to Secretary - Abrievated Graph Key: I415"@en-AU ;
    skos:definition "289  Minister may give directions to Secretary"@en-AU ;
    skos:narrower C2020A00012:410 ;
    skos:prefLabel "Item I415"@en-AU ;
    dcat:accessURL <https://www.legislation.gov.au/C2020A00012/2024-07-10/2024-07-10/text/original/epub/OEBPS/document_1/document_1.html#_Toc172119107> ;
    dcat:landingPage "https://www.legislation.gov.au/C2020A00012/2024-07-10/2024-07-10/text/original/epub/OEBPS/document_1/document_1.html#_Toc172119107"^^xsd:anyURI ;
    dcat:theme legcons:Item .

C2020A00012:418 a legcons:Item,
        owl:Class,
        dcat:Resource ;
    rdfs:label "Item - I418 290  Simplified outline of this Part"@en-AU ;
    dct:isPartOf C2020A00012:417 ;
    dct:isReferencedBy C2020A00012: ;
    rdfs:comment "290  Simplified outline of this Part - Abrievated Graph Key: I418"@en-AU ;
    skos:definition "290  Simplified outline of this Part"@en-AU ;
    skos:narrower C2020A00012:417 ;
    skos:prefLabel "Item I418"@en-AU ;
    dcat:accessURL <https://www.legislation.gov.au/C2020A00012/2024-07-10/2024-07-10/text/original/epub/OEBPS/document_1/document_1.html#_Toc172119110> ;
    dcat:landingPage "https://www.legislation.gov.au/C2020A00012/2024-07-10/2024-07-10/text/original/epub/OEBPS/document_1/document_1.html#_Toc172119110"^^xsd:anyURI ;
    dcat:theme legcons:Item .

C2020A00012:42 a legcons:Item,
        owl:Class,
        dcat:Resource ;
    rdfs:label "Item - I42 29  Rules may prohibit export of prescribed goods subject to conditions"@en-AU ;
    dct:isPartOf C2020A00012:28 ;
    dct:isReferencedBy C2020A00012: ;
    rdfs:comment "29  Rules may prohibit export of prescribed goods subject to conditions - Abrievated Graph Key: I42"@en-AU ;
    skos:definition "29  Rules may prohibit export of prescribed goods subject to conditions"@en-AU ;
    skos:narrower C2020A00012:28 ;
    skos:prefLabel "Item I42"@en-AU ;
    dcat:accessURL <https://www.legislation.gov.au/C2020A00012/2024-07-10/2024-07-10/text/original/epub/OEBPS/document_1/document_1.html#_Toc172118734> ;
    dcat:landingPage "https://www.legislation.gov.au/C2020A00012/2024-07-10/2024-07-10/text/original/epub/OEBPS/document_1/document_1.html#_Toc172118734"^^xsd:anyURI ;
    dcat:theme legcons:Item .

C2020A00012:420 a legcons:Item,
        owl:Class,
        dcat:Resource ;
    rdfs:label "Item - I420 291  Authorisation of persons to be authorised officers"@en-AU ;
    dct:isPartOf C2020A00012:419 ;
    dct:isReferencedBy C2020A00012: ;
    rdfs:comment "291  Authorisation of persons to be authorised officers - Abrievated Graph Key: I420"@en-AU ;
    skos:definition "291  Authorisation of persons to be authorised officers"@en-AU ;
    skos:narrower C2020A00012:419 ;
    skos:prefLabel "Item I420"@en-AU ;
    dcat:accessURL <https://www.legislation.gov.au/C2020A00012/2024-07-10/2024-07-10/text/original/epub/OEBPS/document_1/document_1.html#_Toc172119112> ;
    dcat:landingPage "https://www.legislation.gov.au/C2020A00012/2024-07-10/2024-07-10/text/original/epub/OEBPS/document_1/document_1.html#_Toc172119112"^^xsd:anyURI ;
    dcat:theme legcons:Item .

C2020A00012:421 a legcons:Item,
        owl:Class,
        dcat:Resource ;
    rdfs:label "Item - I421 292  Conditions of authorisation"@en-AU ;
    dct:isPartOf C2020A00012:419 ;
    dct:isReferencedBy C2020A00012: ;
    rdfs:comment "292  Conditions of authorisation - Abrievated Graph Key: I421"@en-AU ;
    skos:definition "292  Conditions of authorisation"@en-AU ;
    skos:narrower C2020A00012:419 ;
    skos:prefLabel "Item I421"@en-AU ;
    dcat:accessURL <https://www.legislation.gov.au/C2020A00012/2024-07-10/2024-07-10/text/original/epub/OEBPS/document_1/document_1.html#_Toc172119113> ;
    dcat:landingPage "https://www.legislation.gov.au/C2020A00012/2024-07-10/2024-07-10/text/original/epub/OEBPS/document_1/document_1.html#_Toc172119113"^^xsd:anyURI ;
    dcat:theme legcons:Item .

C2020A00012:422 a legcons:Item,
        owl:Class,
        dcat:Resource ;
    rdfs:label "Item - I422 293  Third party authorised officers must not contravene conditions of authorisation"@en-AU ;
    dct:isPartOf C2020A00012:419 ;
    dct:isReferencedBy C2020A00012: ;
    rdfs:comment "293  Third party authorised officers must not contravene conditions of authorisation - Abrievated Graph Key: I422"@en-AU ;
    skos:definition "293  Third party authorised officers must not contravene conditions of authorisation"@en-AU ;
    skos:narrower C2020A00012:419 ;
    skos:prefLabel "Item I422"@en-AU ;
    dcat:accessURL <https://www.legislation.gov.au/C2020A00012/2024-07-10/2024-07-10/text/original/epub/OEBPS/document_1/document_1.html#_Toc172119114> ;
    dcat:landingPage "https://www.legislation.gov.au/C2020A00012/2024-07-10/2024-07-10/text/original/epub/OEBPS/document_1/document_1.html#_Toc172119114"^^xsd:anyURI ;
    dcat:theme legcons:Item .

C2020A00012:423 a legcons:Item,
        owl:Class,
        dcat:Resource ;
    rdfs:label "Item - I423 294  Arrangements for State or Territory officers or employees to be authorised officers"@en-AU ;
    dct:isPartOf C2020A00012:419 ;
    dct:isReferencedBy C2020A00012: ;
    rdfs:comment "294  Arrangements for State or Territory officers or employees to be authorised officers - Abrievated Graph Key: I423"@en-AU ;
    skos:definition "294  Arrangements for State or Territory officers or employees to be authorised officers"@en-AU ;
    skos:narrower C2020A00012:419 ;
    skos:prefLabel "Item I423"@en-AU ;
    dcat:accessURL <https://www.legislation.gov.au/C2020A00012/2024-07-10/2024-07-10/text/original/epub/OEBPS/document_1/document_1.html#_Toc172119115> ;
    dcat:landingPage "https://www.legislation.gov.au/C2020A00012/2024-07-10/2024-07-10/text/original/epub/OEBPS/document_1/document_1.html#_Toc172119115"^^xsd:anyURI ;
    dcat:theme legcons:Item .

C2020A00012:426 a legcons:Item,
        owl:Class,
        dcat:Resource ;
    rdfs:label "Item - I426 295  Variation of authorisation"@en-AU ;
    dct:isPartOf C2020A00012:425 ;
    dct:isReferencedBy C2020A00012: ;
    rdfs:comment "295  Variation of authorisation - Abrievated Graph Key: I426"@en-AU ;
    skos:definition "295  Variation of authorisation"@en-AU ;
    skos:narrower C2020A00012:425 ;
    skos:prefLabel "Item I426"@en-AU ;
    dcat:accessURL <https://www.legislation.gov.au/C2020A00012/2024-07-10/2024-07-10/text/original/epub/OEBPS/document_1/document_1.html#_Toc172119118> ;
    dcat:landingPage "https://www.legislation.gov.au/C2020A00012/2024-07-10/2024-07-10/text/original/epub/OEBPS/document_1/document_1.html#_Toc172119118"^^xsd:anyURI ;
    dcat:theme legcons:Item .

C2020A00012:427 a legcons:Item,
        owl:Class,
        dcat:Resource ;
    rdfs:label "Item - I427 296  Suspension of authorisation"@en-AU ;
    dct:isPartOf C2020A00012:425 ;
    dct:isReferencedBy C2020A00012: ;
    rdfs:comment "296  Suspension of authorisation - Abrievated Graph Key: I427"@en-AU ;
    skos:definition "296  Suspension of authorisation"@en-AU ;
    skos:narrower C2020A00012:425 ;
    skos:prefLabel "Item I427"@en-AU ;
    dcat:accessURL <https://www.legislation.gov.au/C2020A00012/2024-07-10/2024-07-10/text/original/epub/OEBPS/document_1/document_1.html#_Toc172119119> ;
    dcat:landingPage "https://www.legislation.gov.au/C2020A00012/2024-07-10/2024-07-10/text/original/epub/OEBPS/document_1/document_1.html#_Toc172119119"^^xsd:anyURI ;
    dcat:theme legcons:Item .

C2020A00012:428 a legcons:Item,
        owl:Class,
        dcat:Resource ;
    rdfs:label "Item - I428 297  Revocation of authorisation"@en-AU ;
    dct:isPartOf C2020A00012:425 ;
    dct:isReferencedBy C2020A00012: ;
    rdfs:comment "297  Revocation of authorisation - Abrievated Graph Key: I428"@en-AU ;
    skos:definition "297  Revocation of authorisation"@en-AU ;
    skos:narrower C2020A00012:425 ;
    skos:prefLabel "Item I428"@en-AU ;
    dcat:accessURL <https://www.legislation.gov.au/C2020A00012/2024-07-10/2024-07-10/text/original/epub/OEBPS/document_1/document_1.html#_Toc172119120> ;
    dcat:landingPage "https://www.legislation.gov.au/C2020A00012/2024-07-10/2024-07-10/text/original/epub/OEBPS/document_1/document_1.html#_Toc172119120"^^xsd:anyURI ;
    dcat:theme legcons:Item .

C2020A00012:429 a legcons:Item,
        owl:Class,
        dcat:Resource ;
    rdfs:label "Item - I429 298  Notice of proposed action must be given to third party authorised officer"@en-AU ;
    dct:isPartOf C2020A00012:425 ;
    dct:isReferencedBy C2020A00012: ;
    rdfs:comment "298  Notice of proposed action must be given to third party authorised officer - Abrievated Graph Key: I429"@en-AU ;
    skos:definition "298  Notice of proposed action must be given to third party authorised officer"@en-AU ;
    skos:narrower C2020A00012:425 ;
    skos:prefLabel "Item I429"@en-AU ;
    dcat:accessURL <https://www.legislation.gov.au/C2020A00012/2024-07-10/2024-07-10/text/original/epub/OEBPS/document_1/document_1.html#_Toc172119121> ;
    dcat:landingPage "https://www.legislation.gov.au/C2020A00012/2024-07-10/2024-07-10/text/original/epub/OEBPS/document_1/document_1.html#_Toc172119121"^^xsd:anyURI ;
    dcat:theme legcons:Item .

C2020A00012:43 a legcons:Division,
        owl:Class,
        dcat:Resource ;
    rdfs:label "Division - D43 Division 4 Offences and civil penalty provisions"@en-AU ;
    dct:isPartOf C2020A00012:28 ;
    dct:isReferencedBy C2020A00012: ;
    rdfs:comment "Division 4 Offences and civil penalty provisions - Abrievated Graph Key: D43"@en-AU ;
    skos:definition "Division 4 Offences and civil penalty provisions"@en-AU ;
    skos:narrower C2020A00012:28 ;
    skos:prefLabel "Division D43"@en-AU ;
    dcat:accessURL <https://www.legislation.gov.au/C2020A00012/2024-07-10/2024-07-10/text/original/epub/OEBPS/document_1/document_1.html#_Toc172118735> ;
    dcat:landingPage "https://www.legislation.gov.au/C2020A00012/2024-07-10/2024-07-10/text/original/epub/OEBPS/document_1/document_1.html#_Toc172118735"^^xsd:anyURI ;
    dcat:theme legcons:Division .

C2020A00012:431 a legcons:Item,
        owl:Class,
        dcat:Resource ;
    rdfs:label "Item - I431 298 A  Application for variation of authorisation"@en-AU ;
    dct:isPartOf C2020A00012:430 ;
    dct:isReferencedBy C2020A00012: ;
    rdfs:comment "298 A  Application for variation of authorisation - Abrievated Graph Key: I431"@en-AU ;
    skos:definition "298 A  Application for variation of authorisation"@en-AU ;
    skos:narrower C2020A00012:430 ;
    skos:prefLabel "Item I431"@en-AU ;
    dcat:accessURL <https://www.legislation.gov.au/C2020A00012/2024-07-10/2024-07-10/text/original/epub/OEBPS/document_1/document_1.html#_Toc172119123> ;
    dcat:landingPage "https://www.legislation.gov.au/C2020A00012/2024-07-10/2024-07-10/text/original/epub/OEBPS/document_1/document_1.html#_Toc172119123"^^xsd:anyURI ;
    dcat:theme legcons:Item .

C2020A00012:432 a legcons:Item,
        owl:Class,
        dcat:Resource ;
    rdfs:label "Item - I432 298 B  Additional or corrected information"@en-AU ;
    dct:isPartOf C2020A00012:430 ;
    dct:isReferencedBy C2020A00012: ;
    rdfs:comment "298 B  Additional or corrected information - Abrievated Graph Key: I432"@en-AU ;
    skos:definition "298 B  Additional or corrected information"@en-AU ;
    skos:narrower C2020A00012:430 ;
    skos:prefLabel "Item I432"@en-AU ;
    dcat:accessURL <https://www.legislation.gov.au/C2020A00012/2024-07-10/2024-07-10/text/original/epub/OEBPS/document_1/document_1.html#_Toc172119124> ;
    dcat:landingPage "https://www.legislation.gov.au/C2020A00012/2024-07-10/2024-07-10/text/original/epub/OEBPS/document_1/document_1.html#_Toc172119124"^^xsd:anyURI ;
    dcat:theme legcons:Item .

C2020A00012:433 a legcons:Item,
        owl:Class,
        dcat:Resource ;
    rdfs:label "Item - I433 298 C  Request for suspension of authorisation"@en-AU ;
    dct:isPartOf C2020A00012:430 ;
    dct:isReferencedBy C2020A00012: ;
    rdfs:comment "298 C  Request for suspension of authorisation - Abrievated Graph Key: I433"@en-AU ;
    skos:definition "298 C  Request for suspension of authorisation"@en-AU ;
    skos:narrower C2020A00012:430 ;
    skos:prefLabel "Item I433"@en-AU ;
    dcat:accessURL <https://www.legislation.gov.au/C2020A00012/2024-07-10/2024-07-10/text/original/epub/OEBPS/document_1/document_1.html#_Toc172119125> ;
    dcat:landingPage "https://www.legislation.gov.au/C2020A00012/2024-07-10/2024-07-10/text/original/epub/OEBPS/document_1/document_1.html#_Toc172119125"^^xsd:anyURI ;
    dcat:theme legcons:Item .

C2020A00012:434 a legcons:Item,
        owl:Class,
        dcat:Resource ;
    rdfs:label "Item - I434 298 D  Request for revocation of authorisation"@en-AU ;
    dct:isPartOf C2020A00012:430 ;
    dct:isReferencedBy C2020A00012: ;
    rdfs:comment "298 D  Request for revocation of authorisation - Abrievated Graph Key: I434"@en-AU ;
    skos:definition "298 D  Request for revocation of authorisation"@en-AU ;
    skos:narrower C2020A00012:430 ;
    skos:prefLabel "Item I434"@en-AU ;
    dcat:accessURL <https://www.legislation.gov.au/C2020A00012/2024-07-10/2024-07-10/text/original/epub/OEBPS/document_1/document_1.html#_Toc172119126> ;
    dcat:landingPage "https://www.legislation.gov.au/C2020A00012/2024-07-10/2024-07-10/text/original/epub/OEBPS/document_1/document_1.html#_Toc172119126"^^xsd:anyURI ;
    dcat:theme legcons:Item .

C2020A00012:436 a legcons:Item,
        owl:Class,
        dcat:Resource ;
    rdfs:label "Item - I436 299  Secretary may request notification of certain events by suspended third party authorised officer"@en-AU ;
    dct:isPartOf C2020A00012:435 ;
    dct:isReferencedBy C2020A00012: ;
    rdfs:comment "299  Secretary may request notification of certain events by suspended third party authorised officer - Abrievated Graph Key: I436"@en-AU ;
    skos:definition "299  Secretary may request notification of certain events by suspended third party authorised officer"@en-AU ;
    skos:narrower C2020A00012:435 ;
    skos:prefLabel "Item I436"@en-AU ;
    dcat:accessURL <https://www.legislation.gov.au/C2020A00012/2024-07-10/2024-07-10/text/original/epub/OEBPS/document_1/document_1.html#_Toc172119128> ;
    dcat:landingPage "https://www.legislation.gov.au/C2020A00012/2024-07-10/2024-07-10/text/original/epub/OEBPS/document_1/document_1.html#_Toc172119128"^^xsd:anyURI ;
    dcat:theme legcons:Item .

C2020A00012:438 a legcons:Item,
        owl:Class,
        dcat:Resource ;
    rdfs:label "Item - I438 300  Rules may confer functions or powers on authorised officers"@en-AU ;
    dct:isPartOf C2020A00012:437 ;
    dct:isReferencedBy C2020A00012: ;
    rdfs:comment "300  Rules may confer functions or powers on authorised officers - Abrievated Graph Key: I438"@en-AU ;
    skos:definition "300  Rules may confer functions or powers on authorised officers"@en-AU ;
    skos:narrower C2020A00012:437 ;
    skos:prefLabel "Item I438"@en-AU ;
    dcat:accessURL <https://www.legislation.gov.au/C2020A00012/2024-07-10/2024-07-10/text/original/epub/OEBPS/document_1/document_1.html#_Toc172119130> ;
    dcat:landingPage "https://www.legislation.gov.au/C2020A00012/2024-07-10/2024-07-10/text/original/epub/OEBPS/document_1/document_1.html#_Toc172119130"^^xsd:anyURI ;
    dcat:theme legcons:Item .

C2020A00012:439 a legcons:Item,
        owl:Class,
        dcat:Resource ;
    rdfs:label "Item - I439 301  Functions and powers of authorised officers"@en-AU ;
    dct:isPartOf C2020A00012:437 ;
    dct:isReferencedBy C2020A00012: ;
    rdfs:comment "301  Functions and powers of authorised officers - Abrievated Graph Key: I439"@en-AU ;
    skos:definition "301  Functions and powers of authorised officers"@en-AU ;
    skos:narrower C2020A00012:437 ;
    skos:prefLabel "Item I439"@en-AU ;
    dcat:accessURL <https://www.legislation.gov.au/C2020A00012/2024-07-10/2024-07-10/text/original/epub/OEBPS/document_1/document_1.html#_Toc172119131> ;
    dcat:landingPage "https://www.legislation.gov.au/C2020A00012/2024-07-10/2024-07-10/text/original/epub/OEBPS/document_1/document_1.html#_Toc172119131"^^xsd:anyURI ;
    dcat:theme legcons:Item .

C2020A00012:44 a legcons:Item,
        owl:Class,
        dcat:Resource ;
    rdfs:label "Item - I44 30  Exporting goods that are subject to prohibition on exportbasic contravention"@en-AU ;
    dct:isPartOf C2020A00012:28 ;
    dct:isReferencedBy C2020A00012: ;
    rdfs:comment "30  Exporting goods that are subject to prohibition on exportbasic contravention - Abrievated Graph Key: I44"@en-AU ;
    skos:definition "30  Exporting goods that are subject to prohibition on exportbasic contravention"@en-AU ;
    skos:narrower C2020A00012:28 ;
    skos:prefLabel "Item I44"@en-AU ;
    dcat:accessURL <https://www.legislation.gov.au/C2020A00012/2024-07-10/2024-07-10/text/original/epub/OEBPS/document_1/document_1.html#_Toc172118736> ;
    dcat:landingPage "https://www.legislation.gov.au/C2020A00012/2024-07-10/2024-07-10/text/original/epub/OEBPS/document_1/document_1.html#_Toc172118736"^^xsd:anyURI ;
    dcat:theme legcons:Item .

C2020A00012:440 a legcons:Item,
        owl:Class,
        dcat:Resource ;
    rdfs:label "Item - I440 302  Third party authorised officer must not contravene direction"@en-AU ;
    dct:isPartOf C2020A00012:437 ;
    dct:isReferencedBy C2020A00012: ;
    rdfs:comment "302  Third party authorised officer must not contravene direction - Abrievated Graph Key: I440"@en-AU ;
    skos:definition "302  Third party authorised officer must not contravene direction"@en-AU ;
    skos:narrower C2020A00012:437 ;
    skos:prefLabel "Item I440"@en-AU ;
    dcat:accessURL <https://www.legislation.gov.au/C2020A00012/2024-07-10/2024-07-10/text/original/epub/OEBPS/document_1/document_1.html#_Toc172119132> ;
    dcat:landingPage "https://www.legislation.gov.au/C2020A00012/2024-07-10/2024-07-10/text/original/epub/OEBPS/document_1/document_1.html#_Toc172119132"^^xsd:anyURI ;
    dcat:theme legcons:Item .

C2020A00012:441 a legcons:Item,
        owl:Class,
        dcat:Resource ;
    rdfs:label "Item - I441 303  Certain authorised officers may charge fees"@en-AU ;
    dct:isPartOf C2020A00012:437 ;
    dct:isReferencedBy C2020A00012: ;
    rdfs:comment "303  Certain authorised officers may charge fees - Abrievated Graph Key: I441"@en-AU ;
    skos:definition "303  Certain authorised officers may charge fees"@en-AU ;
    skos:narrower C2020A00012:437 ;
    skos:prefLabel "Item I441"@en-AU ;
    dcat:accessURL <https://www.legislation.gov.au/C2020A00012/2024-07-10/2024-07-10/text/original/epub/OEBPS/document_1/document_1.html#_Toc172119133> ;
    dcat:landingPage "https://www.legislation.gov.au/C2020A00012/2024-07-10/2024-07-10/text/original/epub/OEBPS/document_1/document_1.html#_Toc172119133"^^xsd:anyURI ;
    dcat:theme legcons:Item .

C2020A00012:442 a legcons:Item,
        owl:Class,
        dcat:Resource ;
    rdfs:label "Item - I442 304  Direction to assist persons performing functions etc under this Act"@en-AU ;
    dct:isPartOf C2020A00012:437 ;
    dct:isReferencedBy C2020A00012: ;
    rdfs:comment "304  Direction to assist persons performing functions etc under this Act - Abrievated Graph Key: I442"@en-AU ;
    skos:definition "304  Direction to assist persons performing functions etc under this Act"@en-AU ;
    skos:narrower C2020A00012:437 ;
    skos:prefLabel "Item I442"@en-AU ;
    dcat:accessURL <https://www.legislation.gov.au/C2020A00012/2024-07-10/2024-07-10/text/original/epub/OEBPS/document_1/document_1.html#_Toc172119134> ;
    dcat:landingPage "https://www.legislation.gov.au/C2020A00012/2024-07-10/2024-07-10/text/original/epub/OEBPS/document_1/document_1.html#_Toc172119134"^^xsd:anyURI ;
    dcat:theme legcons:Item .

C2020A00012:443 a legcons:Item,
        owl:Class,
        dcat:Resource ;
    rdfs:label "Item - I443 305  Direction to deal with non compliance with the requirements of this Act etc"@en-AU ;
    dct:isPartOf C2020A00012:437 ;
    dct:isReferencedBy C2020A00012: ;
    rdfs:comment "305  Direction to deal with non compliance with the requirements of this Act etc - Abrievated Graph Key: I443"@en-AU ;
    skos:definition "305  Direction to deal with non compliance with the requirements of this Act etc"@en-AU ;
    skos:narrower C2020A00012:437 ;
    skos:prefLabel "Item I443"@en-AU ;
    dcat:accessURL <https://www.legislation.gov.au/C2020A00012/2024-07-10/2024-07-10/text/original/epub/OEBPS/document_1/document_1.html#_Toc172119135> ;
    dcat:landingPage "https://www.legislation.gov.au/C2020A00012/2024-07-10/2024-07-10/text/original/epub/OEBPS/document_1/document_1.html#_Toc172119135"^^xsd:anyURI ;
    dcat:theme legcons:Item .

C2020A00012:445 a legcons:Item,
        owl:Class,
        dcat:Resource ;
    rdfs:label "Item - I445 306  Identity cards"@en-AU ;
    dct:isPartOf C2020A00012:444 ;
    dct:isReferencedBy C2020A00012: ;
    rdfs:comment "306  Identity cards - Abrievated Graph Key: I445"@en-AU ;
    skos:definition "306  Identity cards"@en-AU ;
    skos:narrower C2020A00012:444 ;
    skos:prefLabel "Item I445"@en-AU ;
    dcat:accessURL <https://www.legislation.gov.au/C2020A00012/2024-07-10/2024-07-10/text/original/epub/OEBPS/document_1/document_1.html#_Toc172119137> ;
    dcat:landingPage "https://www.legislation.gov.au/C2020A00012/2024-07-10/2024-07-10/text/original/epub/OEBPS/document_1/document_1.html#_Toc172119137"^^xsd:anyURI ;
    dcat:theme legcons:Item .

C2020A00012:446 a legcons:Item,
        owl:Class,
        dcat:Resource ;
    rdfs:label "Item - I446 307  Offencefailure to return identity card"@en-AU ;
    dct:isPartOf C2020A00012:444 ;
    dct:isReferencedBy C2020A00012: ;
    rdfs:comment "307  Offencefailure to return identity card - Abrievated Graph Key: I446"@en-AU ;
    skos:definition "307  Offencefailure to return identity card"@en-AU ;
    skos:narrower C2020A00012:444 ;
    skos:prefLabel "Item I446"@en-AU ;
    dcat:accessURL <https://www.legislation.gov.au/C2020A00012/2024-07-10/2024-07-10/text/original/epub/OEBPS/document_1/document_1.html#_Toc172119138> ;
    dcat:landingPage "https://www.legislation.gov.au/C2020A00012/2024-07-10/2024-07-10/text/original/epub/OEBPS/document_1/document_1.html#_Toc172119138"^^xsd:anyURI ;
    dcat:theme legcons:Item .

C2020A00012:447 a legcons:Item,
        owl:Class,
        dcat:Resource ;
    rdfs:label "Item - I447 308  Certain goods or services must not be provided to or received by authorised officers"@en-AU ;
    dct:isPartOf C2020A00012:444 ;
    dct:isReferencedBy C2020A00012: ;
    rdfs:comment "308  Certain goods or services must not be provided to or received by authorised officers - Abrievated Graph Key: I447"@en-AU ;
    skos:definition "308  Certain goods or services must not be provided to or received by authorised officers"@en-AU ;
    skos:narrower C2020A00012:444 ;
    skos:prefLabel "Item I447"@en-AU ;
    dcat:accessURL <https://www.legislation.gov.au/C2020A00012/2024-07-10/2024-07-10/text/original/epub/OEBPS/document_1/document_1.html#_Toc172119139> ;
    dcat:landingPage "https://www.legislation.gov.au/C2020A00012/2024-07-10/2024-07-10/text/original/epub/OEBPS/document_1/document_1.html#_Toc172119139"^^xsd:anyURI ;
    dcat:theme legcons:Item .

C2020A00012:448 a legcons:Item,
        owl:Class,
        dcat:Resource ;
    rdfs:label "Item - I448 309  General provisions relating to directions"@en-AU ;
    dct:isPartOf C2020A00012:444 ;
    dct:isReferencedBy C2020A00012: ;
    rdfs:comment "309  General provisions relating to directions - Abrievated Graph Key: I448"@en-AU ;
    skos:definition "309  General provisions relating to directions"@en-AU ;
    skos:narrower C2020A00012:444 ;
    skos:prefLabel "Item I448"@en-AU ;
    dcat:accessURL <https://www.legislation.gov.au/C2020A00012/2024-07-10/2024-07-10/text/original/epub/OEBPS/document_1/document_1.html#_Toc172119140> ;
    dcat:landingPage "https://www.legislation.gov.au/C2020A00012/2024-07-10/2024-07-10/text/original/epub/OEBPS/document_1/document_1.html#_Toc172119140"^^xsd:anyURI ;
    dcat:theme legcons:Item .

C2020A00012:45 a legcons:Item,
        owl:Class,
        dcat:Resource ;
    rdfs:label "Item - I45 31  Exporting goods that are subject to prohibition on exportintention to obtain commercial advantage"@en-AU ;
    dct:isPartOf C2020A00012:28 ;
    dct:isReferencedBy C2020A00012: ;
    rdfs:comment "31  Exporting goods that are subject to prohibition on exportintention to obtain commercial advantage - Abrievated Graph Key: I45"@en-AU ;
    skos:definition "31  Exporting goods that are subject to prohibition on exportintention to obtain commercial advantage"@en-AU ;
    skos:narrower C2020A00012:28 ;
    skos:prefLabel "Item I45"@en-AU ;
    dcat:accessURL <https://www.legislation.gov.au/C2020A00012/2024-07-10/2024-07-10/text/original/epub/OEBPS/document_1/document_1.html#_Toc172118737> ;
    dcat:landingPage "https://www.legislation.gov.au/C2020A00012/2024-07-10/2024-07-10/text/original/epub/OEBPS/document_1/document_1.html#_Toc172118737"^^xsd:anyURI ;
    dcat:theme legcons:Item .

C2020A00012:451 a legcons:Item,
        owl:Class,
        dcat:Resource ;
    rdfs:label "Item - I451 310  Simplified outline of this Part"@en-AU ;
    dct:isPartOf C2020A00012:450 ;
    dct:isReferencedBy C2020A00012: ;
    rdfs:comment "310  Simplified outline of this Part - Abrievated Graph Key: I451"@en-AU ;
    skos:definition "310  Simplified outline of this Part"@en-AU ;
    skos:narrower C2020A00012:450 ;
    skos:prefLabel "Item I451"@en-AU ;
    dcat:accessURL <https://www.legislation.gov.au/C2020A00012/2024-07-10/2024-07-10/text/original/epub/OEBPS/document_1/document_1.html#_Toc172119143> ;
    dcat:landingPage "https://www.legislation.gov.au/C2020A00012/2024-07-10/2024-07-10/text/original/epub/OEBPS/document_1/document_1.html#_Toc172119143"^^xsd:anyURI ;
    dcat:theme legcons:Item .

C2020A00012:453 a legcons:Item,
        owl:Class,
        dcat:Resource ;
    rdfs:label "Item - I453 311  Approved export programs"@en-AU ;
    dct:isPartOf C2020A00012:452 ;
    dct:isReferencedBy C2020A00012: ;
    rdfs:comment "311  Approved export programs - Abrievated Graph Key: I453"@en-AU ;
    skos:definition "311  Approved export programs"@en-AU ;
    skos:narrower C2020A00012:452 ;
    skos:prefLabel "Item I453"@en-AU ;
    dcat:accessURL <https://www.legislation.gov.au/C2020A00012/2024-07-10/2024-07-10/text/original/epub/OEBPS/document_1/document_1.html#_Toc172119145> ;
    dcat:landingPage "https://www.legislation.gov.au/C2020A00012/2024-07-10/2024-07-10/text/original/epub/OEBPS/document_1/document_1.html#_Toc172119145"^^xsd:anyURI ;
    dcat:theme legcons:Item .

C2020A00012:454 a legcons:Item,
        owl:Class,
        dcat:Resource ;
    rdfs:label "Item - I454 312  Accreditation of veterinarians"@en-AU ;
    dct:isPartOf C2020A00012:452 ;
    dct:isReferencedBy C2020A00012: ;
    rdfs:comment "312  Accreditation of veterinarians - Abrievated Graph Key: I454"@en-AU ;
    skos:definition "312  Accreditation of veterinarians"@en-AU ;
    skos:narrower C2020A00012:452 ;
    skos:prefLabel "Item I454"@en-AU ;
    dcat:accessURL <https://www.legislation.gov.au/C2020A00012/2024-07-10/2024-07-10/text/original/epub/OEBPS/document_1/document_1.html#_Toc172119146> ;
    dcat:landingPage "https://www.legislation.gov.au/C2020A00012/2024-07-10/2024-07-10/text/original/epub/OEBPS/document_1/document_1.html#_Toc172119146"^^xsd:anyURI ;
    dcat:theme legcons:Item .

C2020A00012:455 a legcons:Item,
        owl:Class,
        dcat:Resource ;
    rdfs:label "Item - I455 313  Secretary may direct authorised officers to carry out certain export operations in approved export program"@en-AU ;
    dct:isPartOf C2020A00012:452 ;
    dct:isReferencedBy C2020A00012: ;
    rdfs:comment "313  Secretary may direct authorised officers to carry out certain export operations in approved export program - Abrievated Graph Key: I455"@en-AU ;
    skos:definition "313  Secretary may direct authorised officers to carry out certain export operations in approved export program"@en-AU ;
    skos:narrower C2020A00012:452 ;
    skos:prefLabel "Item I455"@en-AU ;
    dcat:accessURL <https://www.legislation.gov.au/C2020A00012/2024-07-10/2024-07-10/text/original/epub/OEBPS/document_1/document_1.html#_Toc172119147> ;
    dcat:landingPage "https://www.legislation.gov.au/C2020A00012/2024-07-10/2024-07-10/text/original/epub/OEBPS/document_1/document_1.html#_Toc172119147"^^xsd:anyURI ;
    dcat:theme legcons:Item .

C2020A00012:456 a legcons:Item,
        owl:Class,
        dcat:Resource ;
    rdfs:label "Item - I456 314  Secretary may direct authorised officer to monitor or review export operations in approved export programs"@en-AU ;
    dct:isPartOf C2020A00012:452 ;
    dct:isReferencedBy C2020A00012: ;
    rdfs:comment "314  Secretary may direct authorised officer to monitor or review export operations in approved export programs - Abrievated Graph Key: I456"@en-AU ;
    skos:definition "314  Secretary may direct authorised officer to monitor or review export operations in approved export programs"@en-AU ;
    skos:narrower C2020A00012:452 ;
    skos:prefLabel "Item I456"@en-AU ;
    dcat:accessURL <https://www.legislation.gov.au/C2020A00012/2024-07-10/2024-07-10/text/original/epub/OEBPS/document_1/document_1.html#_Toc172119148> ;
    dcat:landingPage "https://www.legislation.gov.au/C2020A00012/2024-07-10/2024-07-10/text/original/epub/OEBPS/document_1/document_1.html#_Toc172119148"^^xsd:anyURI ;
    dcat:theme legcons:Item .

C2020A00012:458 a legcons:Item,
        owl:Class,
        dcat:Resource ;
    rdfs:label "Item - I458 315  Offenceperson other than accredited veterinarian or authorised officer carrying out export operations in approved export program"@en-AU ;
    dct:isPartOf C2020A00012:457 ;
    dct:isReferencedBy C2020A00012: ;
    rdfs:comment "315  Offenceperson other than accredited veterinarian or authorised officer carrying out export operations in approved export program - Abrievated Graph Key: I458"@en-AU ;
    skos:definition "315  Offenceperson other than accredited veterinarian or authorised officer carrying out export operations in approved export program"@en-AU ;
    skos:narrower C2020A00012:457 ;
    skos:prefLabel "Item I458"@en-AU ;
    dcat:accessURL <https://www.legislation.gov.au/C2020A00012/2024-07-10/2024-07-10/text/original/epub/OEBPS/document_1/document_1.html#_Toc172119150> ;
    dcat:landingPage "https://www.legislation.gov.au/C2020A00012/2024-07-10/2024-07-10/text/original/epub/OEBPS/document_1/document_1.html#_Toc172119150"^^xsd:anyURI ;
    dcat:theme legcons:Item .

C2020A00012:459 a legcons:Item,
        owl:Class,
        dcat:Resource ;
    rdfs:label "Item - I459 316  Strict liability offencefailure to keep records or provide reports in relation to approved export program"@en-AU ;
    dct:isPartOf C2020A00012:457 ;
    dct:isReferencedBy C2020A00012: ;
    rdfs:comment "316  Strict liability offencefailure to keep records or provide reports in relation to approved export program - Abrievated Graph Key: I459"@en-AU ;
    skos:definition "316  Strict liability offencefailure to keep records or provide reports in relation to approved export program"@en-AU ;
    skos:narrower C2020A00012:457 ;
    skos:prefLabel "Item I459"@en-AU ;
    dcat:accessURL <https://www.legislation.gov.au/C2020A00012/2024-07-10/2024-07-10/text/original/epub/OEBPS/document_1/document_1.html#_Toc172119151> ;
    dcat:landingPage "https://www.legislation.gov.au/C2020A00012/2024-07-10/2024-07-10/text/original/epub/OEBPS/document_1/document_1.html#_Toc172119151"^^xsd:anyURI ;
    dcat:theme legcons:Item .

C2020A00012:46 a legcons:Item,
        owl:Class,
        dcat:Resource ;
    rdfs:label "Item - I46 32  Exporting goods that are subject to prohibition on exporteconomic consequences for Australia"@en-AU ;
    dct:isPartOf C2020A00012:28 ;
    dct:isReferencedBy C2020A00012: ;
    rdfs:comment "32  Exporting goods that are subject to prohibition on exporteconomic consequences for Australia - Abrievated Graph Key: I46"@en-AU ;
    skos:definition "32  Exporting goods that are subject to prohibition on exporteconomic consequences for Australia"@en-AU ;
    skos:narrower C2020A00012:28 ;
    skos:prefLabel "Item I46"@en-AU ;
    dcat:accessURL <https://www.legislation.gov.au/C2020A00012/2024-07-10/2024-07-10/text/original/epub/OEBPS/document_1/document_1.html#_Toc172118738> ;
    dcat:landingPage "https://www.legislation.gov.au/C2020A00012/2024-07-10/2024-07-10/text/original/epub/OEBPS/document_1/document_1.html#_Toc172118738"^^xsd:anyURI ;
    dcat:theme legcons:Item .

C2020A00012:460 a legcons:Item,
        owl:Class,
        dcat:Resource ;
    rdfs:label "Item - I460 317  Strict liability offencefailure to remedy deficiency in carrying out approved export program"@en-AU ;
    dct:isPartOf C2020A00012:457 ;
    dct:isReferencedBy C2020A00012: ;
    rdfs:comment "317  Strict liability offencefailure to remedy deficiency in carrying out approved export program - Abrievated Graph Key: I460"@en-AU ;
    skos:definition "317  Strict liability offencefailure to remedy deficiency in carrying out approved export program"@en-AU ;
    skos:narrower C2020A00012:457 ;
    skos:prefLabel "Item I460"@en-AU ;
    dcat:accessURL <https://www.legislation.gov.au/C2020A00012/2024-07-10/2024-07-10/text/original/epub/OEBPS/document_1/document_1.html#_Toc172119152> ;
    dcat:landingPage "https://www.legislation.gov.au/C2020A00012/2024-07-10/2024-07-10/text/original/epub/OEBPS/document_1/document_1.html#_Toc172119152"^^xsd:anyURI ;
    dcat:theme legcons:Item .

C2020A00012:461 a legcons:Item,
        owl:Class,
        dcat:Resource ;
    rdfs:label "Item - I461 318  Offencefailure to ensure accredited veterinarian is engaged to carry out relevant export operations in approved export program"@en-AU ;
    dct:isPartOf C2020A00012:457 ;
    dct:isReferencedBy C2020A00012: ;
    rdfs:comment "318  Offencefailure to ensure accredited veterinarian is engaged to carry out relevant export operations in approved export program - Abrievated Graph Key: I461"@en-AU ;
    skos:definition "318  Offencefailure to ensure accredited veterinarian is engaged to carry out relevant export operations in approved export program"@en-AU ;
    skos:narrower C2020A00012:457 ;
    skos:prefLabel "Item I461"@en-AU ;
    dcat:accessURL <https://www.legislation.gov.au/C2020A00012/2024-07-10/2024-07-10/text/original/epub/OEBPS/document_1/document_1.html#_Toc172119153> ;
    dcat:landingPage "https://www.legislation.gov.au/C2020A00012/2024-07-10/2024-07-10/text/original/epub/OEBPS/document_1/document_1.html#_Toc172119153"^^xsd:anyURI ;
    dcat:theme legcons:Item .

C2020A00012:462 a legcons:Item,
        owl:Class,
        dcat:Resource ;
    rdfs:label "Item - I462 319  Strict liability offencecontravening requirement to allow accredited veterinarian etc to accompany eligible live animals during transport to overseas destination"@en-AU ;
    dct:isPartOf C2020A00012:457 ;
    dct:isReferencedBy C2020A00012: ;
    rdfs:comment "319  Strict liability offencecontravening requirement to allow accredited veterinarian etc to accompany eligible live animals during transport to overseas destination - Abrievated Graph Key: I462"@en-AU ;
    skos:definition "319  Strict liability offencecontravening requirement to allow accredited veterinarian etc to accompany eligible live animals during transport to overseas destination"@en-AU ;
    skos:narrower C2020A00012:457 ;
    skos:prefLabel "Item I462"@en-AU ;
    dcat:accessURL <https://www.legislation.gov.au/C2020A00012/2024-07-10/2024-07-10/text/original/epub/OEBPS/document_1/document_1.html#_Toc172119154> ;
    dcat:landingPage "https://www.legislation.gov.au/C2020A00012/2024-07-10/2024-07-10/text/original/epub/OEBPS/document_1/document_1.html#_Toc172119154"^^xsd:anyURI ;
    dcat:theme legcons:Item .

C2020A00012:463 a legcons:Item,
        owl:Class,
        dcat:Resource ;
    rdfs:label "Item - I463 320  Person must not obstruct or hinder accredited veterinarians etc carrying out export operations in approved export program"@en-AU ;
    dct:isPartOf C2020A00012:457 ;
    dct:isReferencedBy C2020A00012: ;
    rdfs:comment "320  Person must not obstruct or hinder accredited veterinarians etc carrying out export operations in approved export program - Abrievated Graph Key: I463"@en-AU ;
    skos:definition "320  Person must not obstruct or hinder accredited veterinarians etc carrying out export operations in approved export program"@en-AU ;
    skos:narrower C2020A00012:457 ;
    skos:prefLabel "Item I463"@en-AU ;
    dcat:accessURL <https://www.legislation.gov.au/C2020A00012/2024-07-10/2024-07-10/text/original/epub/OEBPS/document_1/document_1.html#_Toc172119155> ;
    dcat:landingPage "https://www.legislation.gov.au/C2020A00012/2024-07-10/2024-07-10/text/original/epub/OEBPS/document_1/document_1.html#_Toc172119155"^^xsd:anyURI ;
    dcat:theme legcons:Item .

C2020A00012:464 a legcons:Item,
        owl:Class,
        dcat:Resource ;
    rdfs:label "Item - I464 321  Strict liability offencecontravening requirement to provide reasonable facilities and assistance to accredited veterinarian etc"@en-AU ;
    dct:isPartOf C2020A00012:457 ;
    dct:isReferencedBy C2020A00012: ;
    rdfs:comment "321  Strict liability offencecontravening requirement to provide reasonable facilities and assistance to accredited veterinarian etc - Abrievated Graph Key: I464"@en-AU ;
    skos:definition "321  Strict liability offencecontravening requirement to provide reasonable facilities and assistance to accredited veterinarian etc"@en-AU ;
    skos:narrower C2020A00012:457 ;
    skos:prefLabel "Item I464"@en-AU ;
    dcat:accessURL <https://www.legislation.gov.au/C2020A00012/2024-07-10/2024-07-10/text/original/epub/OEBPS/document_1/document_1.html#_Toc172119156> ;
    dcat:landingPage "https://www.legislation.gov.au/C2020A00012/2024-07-10/2024-07-10/text/original/epub/OEBPS/document_1/document_1.html#_Toc172119156"^^xsd:anyURI ;
    dcat:theme legcons:Item .

C2020A00012:466 a legcons:Item,
        owl:Class,
        dcat:Resource ;
    rdfs:label "Item - I466 322  Extended geographical operation of offences"@en-AU ;
    dct:isPartOf C2020A00012:465 ;
    dct:isReferencedBy C2020A00012: ;
    rdfs:comment "322  Extended geographical operation of offences - Abrievated Graph Key: I466"@en-AU ;
    skos:definition "322  Extended geographical operation of offences"@en-AU ;
    skos:narrower C2020A00012:465 ;
    skos:prefLabel "Item I466"@en-AU ;
    dcat:accessURL <https://www.legislation.gov.au/C2020A00012/2024-07-10/2024-07-10/text/original/epub/OEBPS/document_1/document_1.html#_Toc172119158> ;
    dcat:landingPage "https://www.legislation.gov.au/C2020A00012/2024-07-10/2024-07-10/text/original/epub/OEBPS/document_1/document_1.html#_Toc172119158"^^xsd:anyURI ;
    dcat:theme legcons:Item .

C2020A00012:469 a legcons:Item,
        owl:Class,
        dcat:Resource ;
    rdfs:label "Item - I469 323  Simplified outline of this Part"@en-AU ;
    dct:isPartOf C2020A00012:468 ;
    dct:isReferencedBy C2020A00012: ;
    rdfs:comment "323  Simplified outline of this Part - Abrievated Graph Key: I469"@en-AU ;
    skos:definition "323  Simplified outline of this Part"@en-AU ;
    skos:narrower C2020A00012:468 ;
    skos:prefLabel "Item I469"@en-AU ;
    dcat:accessURL <https://www.legislation.gov.au/C2020A00012/2024-07-10/2024-07-10/text/original/epub/OEBPS/document_1/document_1.html#_Toc172119161> ;
    dcat:landingPage "https://www.legislation.gov.au/C2020A00012/2024-07-10/2024-07-10/text/original/epub/OEBPS/document_1/document_1.html#_Toc172119161"^^xsd:anyURI ;
    dcat:theme legcons:Item .

C2020A00012:47 a legcons:Item,
        owl:Class,
        dcat:Resource ;
    rdfs:label "Item - I47 33  Conveying or possessing goods that are subject to prohibition on export and are intended to be exported etc"@en-AU ;
    dct:isPartOf C2020A00012:28 ;
    dct:isReferencedBy C2020A00012: ;
    rdfs:comment "33  Conveying or possessing goods that are subject to prohibition on export and are intended to be exported etc - Abrievated Graph Key: I47"@en-AU ;
    skos:definition "33  Conveying or possessing goods that are subject to prohibition on export and are intended to be exported etc"@en-AU ;
    skos:narrower C2020A00012:28 ;
    skos:prefLabel "Item I47"@en-AU ;
    dcat:accessURL <https://www.legislation.gov.au/C2020A00012/2024-07-10/2024-07-10/text/original/epub/OEBPS/document_1/document_1.html#_Toc172118739> ;
    dcat:landingPage "https://www.legislation.gov.au/C2020A00012/2024-07-10/2024-07-10/text/original/epub/OEBPS/document_1/document_1.html#_Toc172118739"^^xsd:anyURI ;
    dcat:theme legcons:Item .

C2020A00012:470 a legcons:Item,
        owl:Class,
        dcat:Resource ;
    rdfs:label "Item - I470 324  Modified meaning of authorised officer"@en-AU ;
    dct:isPartOf C2020A00012:468 ;
    dct:isReferencedBy C2020A00012: ;
    rdfs:comment "324  Modified meaning of authorised officer - Abrievated Graph Key: I470"@en-AU ;
    skos:definition "324  Modified meaning of authorised officer"@en-AU ;
    skos:narrower C2020A00012:468 ;
    skos:prefLabel "Item I470"@en-AU ;
    dcat:accessURL <https://www.legislation.gov.au/C2020A00012/2024-07-10/2024-07-10/text/original/epub/OEBPS/document_1/document_1.html#_Toc172119162> ;
    dcat:landingPage "https://www.legislation.gov.au/C2020A00012/2024-07-10/2024-07-10/text/original/epub/OEBPS/document_1/document_1.html#_Toc172119162"^^xsd:anyURI ;
    dcat:theme legcons:Item .

C2020A00012:473 a legcons:Item,
        owl:Class,
        dcat:Resource ;
    rdfs:label "Item - I473 325  Simplified outline of this Part"@en-AU ;
    dct:isPartOf C2020A00012:472 ;
    dct:isReferencedBy C2020A00012: ;
    rdfs:comment "325  Simplified outline of this Part - Abrievated Graph Key: I473"@en-AU ;
    skos:definition "325  Simplified outline of this Part"@en-AU ;
    skos:narrower C2020A00012:472 ;
    skos:prefLabel "Item I473"@en-AU ;
    dcat:accessURL <https://www.legislation.gov.au/C2020A00012/2024-07-10/2024-07-10/text/original/epub/OEBPS/document_1/document_1.html#_Toc172119165> ;
    dcat:landingPage "https://www.legislation.gov.au/C2020A00012/2024-07-10/2024-07-10/text/original/epub/OEBPS/document_1/document_1.html#_Toc172119165"^^xsd:anyURI ;
    dcat:theme legcons:Item .

C2020A00012:475 a legcons:Item,
        owl:Class,
        dcat:Resource ;
    rdfs:label "Item - I475 326  Basic monitoring powers under Part 2 of the Regulatory Powers Act"@en-AU ;
    dct:isPartOf C2020A00012:474 ;
    dct:isReferencedBy C2020A00012: ;
    rdfs:comment "326  Basic monitoring powers under Part 2 of the Regulatory Powers Act - Abrievated Graph Key: I475"@en-AU ;
    skos:definition "326  Basic monitoring powers under Part 2 of the Regulatory Powers Act"@en-AU ;
    skos:narrower C2020A00012:474 ;
    skos:prefLabel "Item I475"@en-AU ;
    dcat:accessURL <https://www.legislation.gov.au/C2020A00012/2024-07-10/2024-07-10/text/original/epub/OEBPS/document_1/document_1.html#_Toc172119167> ;
    dcat:landingPage "https://www.legislation.gov.au/C2020A00012/2024-07-10/2024-07-10/text/original/epub/OEBPS/document_1/document_1.html#_Toc172119167"^^xsd:anyURI ;
    dcat:theme legcons:Item .

C2020A00012:476 a legcons:Item,
        owl:Class,
        dcat:Resource ;
    rdfs:label "Item - I476 327  Modifications of Part 2 of the Regulatory Powers Act"@en-AU ;
    dct:isPartOf C2020A00012:474 ;
    dct:isReferencedBy C2020A00012: ;
    rdfs:comment "327  Modifications of Part 2 of the Regulatory Powers Act - Abrievated Graph Key: I476"@en-AU ;
    skos:definition "327  Modifications of Part 2 of the Regulatory Powers Act"@en-AU ;
    skos:narrower C2020A00012:474 ;
    skos:prefLabel "Item I476"@en-AU ;
    dcat:accessURL <https://www.legislation.gov.au/C2020A00012/2024-07-10/2024-07-10/text/original/epub/OEBPS/document_1/document_1.html#_Toc172119168> ;
    dcat:landingPage "https://www.legislation.gov.au/C2020A00012/2024-07-10/2024-07-10/text/original/epub/OEBPS/document_1/document_1.html#_Toc172119168"^^xsd:anyURI ;
    dcat:theme legcons:Item .

C2020A00012:479 a legcons:Item,
        owl:Class,
        dcat:Resource ;
    rdfs:label "Item - I479 328  Simplified outline of this Part"@en-AU ;
    dct:isPartOf C2020A00012:478 ;
    dct:isReferencedBy C2020A00012: ;
    rdfs:comment "328  Simplified outline of this Part - Abrievated Graph Key: I479"@en-AU ;
    skos:definition "328  Simplified outline of this Part"@en-AU ;
    skos:narrower C2020A00012:478 ;
    skos:prefLabel "Item I479"@en-AU ;
    dcat:accessURL <https://www.legislation.gov.au/C2020A00012/2024-07-10/2024-07-10/text/original/epub/OEBPS/document_1/document_1.html#_Toc172119171> ;
    dcat:landingPage "https://www.legislation.gov.au/C2020A00012/2024-07-10/2024-07-10/text/original/epub/OEBPS/document_1/document_1.html#_Toc172119171"^^xsd:anyURI ;
    dcat:theme legcons:Item .

C2020A00012:48 a legcons:Item,
        owl:Class,
        dcat:Resource ;
    rdfs:label "Item - I48 34  Exporting goods to a temporarily prohibited placebasic contravention"@en-AU ;
    dct:isPartOf C2020A00012:28 ;
    dct:isReferencedBy C2020A00012: ;
    rdfs:comment "34  Exporting goods to a temporarily prohibited placebasic contravention - Abrievated Graph Key: I48"@en-AU ;
    skos:definition "34  Exporting goods to a temporarily prohibited placebasic contravention"@en-AU ;
    skos:narrower C2020A00012:28 ;
    skos:prefLabel "Item I48"@en-AU ;
    dcat:accessURL <https://www.legislation.gov.au/C2020A00012/2024-07-10/2024-07-10/text/original/epub/OEBPS/document_1/document_1.html#_Toc172118740> ;
    dcat:landingPage "https://www.legislation.gov.au/C2020A00012/2024-07-10/2024-07-10/text/original/epub/OEBPS/document_1/document_1.html#_Toc172118740"^^xsd:anyURI ;
    dcat:theme legcons:Item .

C2020A00012:481 a legcons:Item,
        owl:Class,
        dcat:Resource ;
    rdfs:label "Item - I481 329  Basic investigation powers under Part 3 of the Regulatory Powers Act"@en-AU ;
    dct:isPartOf C2020A00012:480 ;
    dct:isReferencedBy C2020A00012: ;
    rdfs:comment "329  Basic investigation powers under Part 3 of the Regulatory Powers Act - Abrievated Graph Key: I481"@en-AU ;
    skos:definition "329  Basic investigation powers under Part 3 of the Regulatory Powers Act"@en-AU ;
    skos:narrower C2020A00012:480 ;
    skos:prefLabel "Item I481"@en-AU ;
    dcat:accessURL <https://www.legislation.gov.au/C2020A00012/2024-07-10/2024-07-10/text/original/epub/OEBPS/document_1/document_1.html#_Toc172119173> ;
    dcat:landingPage "https://www.legislation.gov.au/C2020A00012/2024-07-10/2024-07-10/text/original/epub/OEBPS/document_1/document_1.html#_Toc172119173"^^xsd:anyURI ;
    dcat:theme legcons:Item .

C2020A00012:482 a legcons:Item,
        owl:Class,
        dcat:Resource ;
    rdfs:label "Item - I482 330  Modifications of Part 3 of the Regulatory Powers Act"@en-AU ;
    dct:isPartOf C2020A00012:480 ;
    dct:isReferencedBy C2020A00012: ;
    rdfs:comment "330  Modifications of Part 3 of the Regulatory Powers Act - Abrievated Graph Key: I482"@en-AU ;
    skos:definition "330  Modifications of Part 3 of the Regulatory Powers Act"@en-AU ;
    skos:narrower C2020A00012:480 ;
    skos:prefLabel "Item I482"@en-AU ;
    dcat:accessURL <https://www.legislation.gov.au/C2020A00012/2024-07-10/2024-07-10/text/original/epub/OEBPS/document_1/document_1.html#_Toc172119174> ;
    dcat:landingPage "https://www.legislation.gov.au/C2020A00012/2024-07-10/2024-07-10/text/original/epub/OEBPS/document_1/document_1.html#_Toc172119174"^^xsd:anyURI ;
    dcat:theme legcons:Item .

C2020A00012:485 a legcons:Item,
        owl:Class,
        dcat:Resource ;
    rdfs:label "Item - I485 331  Simplified outline of this Part"@en-AU ;
    dct:isPartOf C2020A00012:484 ;
    dct:isReferencedBy C2020A00012: ;
    rdfs:comment "331  Simplified outline of this Part - Abrievated Graph Key: I485"@en-AU ;
    skos:definition "331  Simplified outline of this Part"@en-AU ;
    skos:narrower C2020A00012:484 ;
    skos:prefLabel "Item I485"@en-AU ;
    dcat:accessURL <https://www.legislation.gov.au/C2020A00012/2024-07-10/2024-07-10/text/original/epub/OEBPS/document_1/document_1.html#_Toc172119177> ;
    dcat:landingPage "https://www.legislation.gov.au/C2020A00012/2024-07-10/2024-07-10/text/original/epub/OEBPS/document_1/document_1.html#_Toc172119177"^^xsd:anyURI ;
    dcat:theme legcons:Item .

C2020A00012:486 a legcons:Item,
        owl:Class,
        dcat:Resource ;
    rdfs:label "Item - I486 332  Modified meaning of premises"@en-AU ;
    dct:isPartOf C2020A00012:484 ;
    dct:isReferencedBy C2020A00012: ;
    rdfs:comment "332  Modified meaning of premises - Abrievated Graph Key: I486"@en-AU ;
    skos:definition "332  Modified meaning of premises"@en-AU ;
    skos:narrower C2020A00012:484 ;
    skos:prefLabel "Item I486"@en-AU ;
    dcat:accessURL <https://www.legislation.gov.au/C2020A00012/2024-07-10/2024-07-10/text/original/epub/OEBPS/document_1/document_1.html#_Toc172119178> ;
    dcat:landingPage "https://www.legislation.gov.au/C2020A00012/2024-07-10/2024-07-10/text/original/epub/OEBPS/document_1/document_1.html#_Toc172119178"^^xsd:anyURI ;
    dcat:theme legcons:Item .

C2020A00012:488 a legcons:Item,
        owl:Class,
        dcat:Resource ;
    rdfs:label "Item - I488 333  Entering adjacent premises to gain access to other premises"@en-AU ;
    dct:isPartOf C2020A00012:487 ;
    dct:isReferencedBy C2020A00012: ;
    rdfs:comment "333  Entering adjacent premises to gain access to other premises - Abrievated Graph Key: I488"@en-AU ;
    skos:definition "333  Entering adjacent premises to gain access to other premises"@en-AU ;
    skos:narrower C2020A00012:487 ;
    skos:prefLabel "Item I488"@en-AU ;
    dcat:accessURL <https://www.legislation.gov.au/C2020A00012/2024-07-10/2024-07-10/text/original/epub/OEBPS/document_1/document_1.html#_Toc172119180> ;
    dcat:landingPage "https://www.legislation.gov.au/C2020A00012/2024-07-10/2024-07-10/text/original/epub/OEBPS/document_1/document_1.html#_Toc172119180"^^xsd:anyURI ;
    dcat:theme legcons:Item .

C2020A00012:489 a legcons:Item,
        owl:Class,
        dcat:Resource ;
    rdfs:label "Item - I489 334  Entry under adjacent premises warrant"@en-AU ;
    dct:isPartOf C2020A00012:487 ;
    dct:isReferencedBy C2020A00012: ;
    rdfs:comment "334  Entry under adjacent premises warrant - Abrievated Graph Key: I489"@en-AU ;
    skos:definition "334  Entry under adjacent premises warrant"@en-AU ;
    skos:narrower C2020A00012:487 ;
    skos:prefLabel "Item I489"@en-AU ;
    dcat:accessURL <https://www.legislation.gov.au/C2020A00012/2024-07-10/2024-07-10/text/original/epub/OEBPS/document_1/document_1.html#_Toc172119181> ;
    dcat:landingPage "https://www.legislation.gov.au/C2020A00012/2024-07-10/2024-07-10/text/original/epub/OEBPS/document_1/document_1.html#_Toc172119181"^^xsd:anyURI ;
    dcat:theme legcons:Item .

C2020A00012:49 a legcons:Item,
        owl:Class,
        dcat:Resource ;
    rdfs:label "Item - I49 35  Exporting goods to a temporarily prohibited placeintention to obtain commercial advantage"@en-AU ;
    dct:isPartOf C2020A00012:28 ;
    dct:isReferencedBy C2020A00012: ;
    rdfs:comment "35  Exporting goods to a temporarily prohibited placeintention to obtain commercial advantage - Abrievated Graph Key: I49"@en-AU ;
    skos:definition "35  Exporting goods to a temporarily prohibited placeintention to obtain commercial advantage"@en-AU ;
    skos:narrower C2020A00012:28 ;
    skos:prefLabel "Item I49"@en-AU ;
    dcat:accessURL <https://www.legislation.gov.au/C2020A00012/2024-07-10/2024-07-10/text/original/epub/OEBPS/document_1/document_1.html#_Toc172118741> ;
    dcat:landingPage "https://www.legislation.gov.au/C2020A00012/2024-07-10/2024-07-10/text/original/epub/OEBPS/document_1/document_1.html#_Toc172118741"^^xsd:anyURI ;
    dcat:theme legcons:Item .

C2020A00012:491 a legcons:Item,
        owl:Class,
        dcat:Resource ;
    rdfs:label "Item - I491 335  Application and issue of adjacent premises warrant"@en-AU ;
    dct:isPartOf C2020A00012:490 ;
    dct:isReferencedBy C2020A00012: ;
    rdfs:comment "335  Application and issue of adjacent premises warrant - Abrievated Graph Key: I491"@en-AU ;
    skos:definition "335  Application and issue of adjacent premises warrant"@en-AU ;
    skos:narrower C2020A00012:490 ;
    skos:prefLabel "Item I491"@en-AU ;
    dcat:accessURL <https://www.legislation.gov.au/C2020A00012/2024-07-10/2024-07-10/text/original/epub/OEBPS/document_1/document_1.html#_Toc172119183> ;
    dcat:landingPage "https://www.legislation.gov.au/C2020A00012/2024-07-10/2024-07-10/text/original/epub/OEBPS/document_1/document_1.html#_Toc172119183"^^xsd:anyURI ;
    dcat:theme legcons:Item .

C2020A00012:493 a legcons:Item,
        owl:Class,
        dcat:Resource ;
    rdfs:label "Item - I493 336  Consent"@en-AU ;
    dct:isPartOf C2020A00012:492 ;
    dct:isReferencedBy C2020A00012: ;
    rdfs:comment "336  Consent - Abrievated Graph Key: I493"@en-AU ;
    skos:definition "336  Consent"@en-AU ;
    skos:narrower C2020A00012:492 ;
    skos:prefLabel "Item I493"@en-AU ;
    dcat:accessURL <https://www.legislation.gov.au/C2020A00012/2024-07-10/2024-07-10/text/original/epub/OEBPS/document_1/document_1.html#_Toc172119185> ;
    dcat:landingPage "https://www.legislation.gov.au/C2020A00012/2024-07-10/2024-07-10/text/original/epub/OEBPS/document_1/document_1.html#_Toc172119185"^^xsd:anyURI ;
    dcat:theme legcons:Item .

C2020A00012:494 a legcons:Item,
        owl:Class,
        dcat:Resource ;
    rdfs:label "Item - I494 337  Announcement before entry under warrant"@en-AU ;
    dct:isPartOf C2020A00012:492 ;
    dct:isReferencedBy C2020A00012: ;
    rdfs:comment "337  Announcement before entry under warrant - Abrievated Graph Key: I494"@en-AU ;
    skos:definition "337  Announcement before entry under warrant"@en-AU ;
    skos:narrower C2020A00012:492 ;
    skos:prefLabel "Item I494"@en-AU ;
    dcat:accessURL <https://www.legislation.gov.au/C2020A00012/2024-07-10/2024-07-10/text/original/epub/OEBPS/document_1/document_1.html#_Toc172119186> ;
    dcat:landingPage "https://www.legislation.gov.au/C2020A00012/2024-07-10/2024-07-10/text/original/epub/OEBPS/document_1/document_1.html#_Toc172119186"^^xsd:anyURI ;
    dcat:theme legcons:Item .

C2020A00012:495 a legcons:Item,
        owl:Class,
        dcat:Resource ;
    rdfs:label "Item - I495 338  Authorised officer to be in possession of warrant"@en-AU ;
    dct:isPartOf C2020A00012:492 ;
    dct:isReferencedBy C2020A00012: ;
    rdfs:comment "338  Authorised officer to be in possession of warrant - Abrievated Graph Key: I495"@en-AU ;
    skos:definition "338  Authorised officer to be in possession of warrant"@en-AU ;
    skos:narrower C2020A00012:492 ;
    skos:prefLabel "Item I495"@en-AU ;
    dcat:accessURL <https://www.legislation.gov.au/C2020A00012/2024-07-10/2024-07-10/text/original/epub/OEBPS/document_1/document_1.html#_Toc172119187> ;
    dcat:landingPage "https://www.legislation.gov.au/C2020A00012/2024-07-10/2024-07-10/text/original/epub/OEBPS/document_1/document_1.html#_Toc172119187"^^xsd:anyURI ;
    dcat:theme legcons:Item .

C2020A00012:496 a legcons:Item,
        owl:Class,
        dcat:Resource ;
    rdfs:label "Item - I496 339  Details of warrant etc to be provided"@en-AU ;
    dct:isPartOf C2020A00012:492 ;
    dct:isReferencedBy C2020A00012: ;
    rdfs:comment "339  Details of warrant etc to be provided - Abrievated Graph Key: I496"@en-AU ;
    skos:definition "339  Details of warrant etc to be provided"@en-AU ;
    skos:narrower C2020A00012:492 ;
    skos:prefLabel "Item I496"@en-AU ;
    dcat:accessURL <https://www.legislation.gov.au/C2020A00012/2024-07-10/2024-07-10/text/original/epub/OEBPS/document_1/document_1.html#_Toc172119188> ;
    dcat:landingPage "https://www.legislation.gov.au/C2020A00012/2024-07-10/2024-07-10/text/original/epub/OEBPS/document_1/document_1.html#_Toc172119188"^^xsd:anyURI ;
    dcat:theme legcons:Item .

C2020A00012:497 a legcons:Item,
        owl:Class,
        dcat:Resource ;
    rdfs:label "Item - I497 340  Use of force in executing a warrant"@en-AU ;
    dct:isPartOf C2020A00012:492 ;
    dct:isReferencedBy C2020A00012: ;
    rdfs:comment "340  Use of force in executing a warrant - Abrievated Graph Key: I497"@en-AU ;
    skos:definition "340  Use of force in executing a warrant"@en-AU ;
    skos:narrower C2020A00012:492 ;
    skos:prefLabel "Item I497"@en-AU ;
    dcat:accessURL <https://www.legislation.gov.au/C2020A00012/2024-07-10/2024-07-10/text/original/epub/OEBPS/document_1/document_1.html#_Toc172119189> ;
    dcat:landingPage "https://www.legislation.gov.au/C2020A00012/2024-07-10/2024-07-10/text/original/epub/OEBPS/document_1/document_1.html#_Toc172119189"^^xsd:anyURI ;
    dcat:theme legcons:Item .

C2020A00012:499 a legcons:Item,
        owl:Class,
        dcat:Resource ;
    rdfs:label "Item - I499 341  Right to observe execution of warrant"@en-AU ;
    dct:isPartOf C2020A00012:498 ;
    dct:isReferencedBy C2020A00012: ;
    rdfs:comment "341  Right to observe execution of warrant - Abrievated Graph Key: I499"@en-AU ;
    skos:definition "341  Right to observe execution of warrant"@en-AU ;
    skos:narrower C2020A00012:498 ;
    skos:prefLabel "Item I499"@en-AU ;
    dcat:accessURL <https://www.legislation.gov.au/C2020A00012/2024-07-10/2024-07-10/text/original/epub/OEBPS/document_1/document_1.html#_Toc172119191> ;
    dcat:landingPage "https://www.legislation.gov.au/C2020A00012/2024-07-10/2024-07-10/text/original/epub/OEBPS/document_1/document_1.html#_Toc172119191"^^xsd:anyURI ;
    dcat:theme legcons:Item .

C2020A00012:5 a legcons:Item,
        owl:Class,
        dcat:Resource ;
    rdfs:label "Item - I5 3  Objects of this Act"@en-AU ;
    dct:isPartOf C2020A00012:1 ;
    dct:isReferencedBy C2020A00012: ;
    rdfs:comment "3  Objects of this Act - Abrievated Graph Key: I5"@en-AU ;
    skos:definition "3  Objects of this Act"@en-AU ;
    skos:narrower C2020A00012:1 ;
    skos:prefLabel "Item I5"@en-AU ;
    dcat:accessURL <https://www.legislation.gov.au/C2020A00012/2024-07-10/2024-07-10/text/original/epub/OEBPS/document_1/document_1.html#_Toc172118697> ;
    dcat:landingPage "https://www.legislation.gov.au/C2020A00012/2024-07-10/2024-07-10/text/original/epub/OEBPS/document_1/document_1.html#_Toc172118697"^^xsd:anyURI ;
    dcat:theme legcons:Item .

C2020A00012:50 a legcons:Item,
        owl:Class,
        dcat:Resource ;
    rdfs:label "Item - I50 36  Exporting goods to a temporarily prohibited placeeconomic consequences for Australia"@en-AU ;
    dct:isPartOf C2020A00012:28 ;
    dct:isReferencedBy C2020A00012: ;
    rdfs:comment "36  Exporting goods to a temporarily prohibited placeeconomic consequences for Australia - Abrievated Graph Key: I50"@en-AU ;
    skos:definition "36  Exporting goods to a temporarily prohibited placeeconomic consequences for Australia"@en-AU ;
    skos:narrower C2020A00012:28 ;
    skos:prefLabel "Item I50"@en-AU ;
    dcat:accessURL <https://www.legislation.gov.au/C2020A00012/2024-07-10/2024-07-10/text/original/epub/OEBPS/document_1/document_1.html#_Toc172118742> ;
    dcat:landingPage "https://www.legislation.gov.au/C2020A00012/2024-07-10/2024-07-10/text/original/epub/OEBPS/document_1/document_1.html#_Toc172118742"^^xsd:anyURI ;
    dcat:theme legcons:Item .

C2020A00012:500 a legcons:Item,
        owl:Class,
        dcat:Resource ;
    rdfs:label "Item - I500 342  Responsibility to provide facilities and assistance"@en-AU ;
    dct:isPartOf C2020A00012:498 ;
    dct:isReferencedBy C2020A00012: ;
    rdfs:comment "342  Responsibility to provide facilities and assistance - Abrievated Graph Key: I500"@en-AU ;
    skos:definition "342  Responsibility to provide facilities and assistance"@en-AU ;
    skos:narrower C2020A00012:498 ;
    skos:prefLabel "Item I500"@en-AU ;
    dcat:accessURL <https://www.legislation.gov.au/C2020A00012/2024-07-10/2024-07-10/text/original/epub/OEBPS/document_1/document_1.html#_Toc172119192> ;
    dcat:landingPage "https://www.legislation.gov.au/C2020A00012/2024-07-10/2024-07-10/text/original/epub/OEBPS/document_1/document_1.html#_Toc172119192"^^xsd:anyURI ;
    dcat:theme legcons:Item .

C2020A00012:502 a legcons:Item,
        owl:Class,
        dcat:Resource ;
    rdfs:label "Item - I502 343  Powers of issuing officers"@en-AU ;
    dct:isPartOf C2020A00012:501 ;
    dct:isReferencedBy C2020A00012: ;
    rdfs:comment "343  Powers of issuing officers - Abrievated Graph Key: I502"@en-AU ;
    skos:definition "343  Powers of issuing officers"@en-AU ;
    skos:narrower C2020A00012:501 ;
    skos:prefLabel "Item I502"@en-AU ;
    dcat:accessURL <https://www.legislation.gov.au/C2020A00012/2024-07-10/2024-07-10/text/original/epub/OEBPS/document_1/document_1.html#_Toc172119194> ;
    dcat:landingPage "https://www.legislation.gov.au/C2020A00012/2024-07-10/2024-07-10/text/original/epub/OEBPS/document_1/document_1.html#_Toc172119194"^^xsd:anyURI ;
    dcat:theme legcons:Item .

C2020A00012:505 a legcons:Item,
        owl:Class,
        dcat:Resource ;
    rdfs:label "Item - I505 344  Simplified outline of this Part"@en-AU ;
    dct:isPartOf C2020A00012:504 ;
    dct:isReferencedBy C2020A00012: ;
    rdfs:comment "344  Simplified outline of this Part - Abrievated Graph Key: I505"@en-AU ;
    skos:definition "344  Simplified outline of this Part"@en-AU ;
    skos:narrower C2020A00012:504 ;
    skos:prefLabel "Item I505"@en-AU ;
    dcat:accessURL <https://www.legislation.gov.au/C2020A00012/2024-07-10/2024-07-10/text/original/epub/OEBPS/document_1/document_1.html#_Toc172119197> ;
    dcat:landingPage "https://www.legislation.gov.au/C2020A00012/2024-07-10/2024-07-10/text/original/epub/OEBPS/document_1/document_1.html#_Toc172119197"^^xsd:anyURI ;
    dcat:theme legcons:Item .

C2020A00012:506 a legcons:Item,
        owl:Class,
        dcat:Resource ;
    rdfs:label "Item - I506 345  Premises to which this Part applies"@en-AU ;
    dct:isPartOf C2020A00012:504 ;
    dct:isReferencedBy C2020A00012: ;
    rdfs:comment "345  Premises to which this Part applies - Abrievated Graph Key: I506"@en-AU ;
    skos:definition "345  Premises to which this Part applies"@en-AU ;
    skos:narrower C2020A00012:504 ;
    skos:prefLabel "Item I506"@en-AU ;
    dcat:accessURL <https://www.legislation.gov.au/C2020A00012/2024-07-10/2024-07-10/text/original/epub/OEBPS/document_1/document_1.html#_Toc172119198> ;
    dcat:landingPage "https://www.legislation.gov.au/C2020A00012/2024-07-10/2024-07-10/text/original/epub/OEBPS/document_1/document_1.html#_Toc172119198"^^xsd:anyURI ;
    dcat:theme legcons:Item .

C2020A00012:508 a legcons:Item,
        owl:Class,
        dcat:Resource ;
    rdfs:label "Item - I508 346  Monitoring relevant premises"@en-AU ;
    dct:isPartOf C2020A00012:507 ;
    dct:isReferencedBy C2020A00012: ;
    rdfs:comment "346  Monitoring relevant premises - Abrievated Graph Key: I508"@en-AU ;
    skos:definition "346  Monitoring relevant premises"@en-AU ;
    skos:narrower C2020A00012:507 ;
    skos:prefLabel "Item I508"@en-AU ;
    dcat:accessURL <https://www.legislation.gov.au/C2020A00012/2024-07-10/2024-07-10/text/original/epub/OEBPS/document_1/document_1.html#_Toc172119200> ;
    dcat:landingPage "https://www.legislation.gov.au/C2020A00012/2024-07-10/2024-07-10/text/original/epub/OEBPS/document_1/document_1.html#_Toc172119200"^^xsd:anyURI ;
    dcat:theme legcons:Item .

C2020A00012:509 a legcons:Item,
        owl:Class,
        dcat:Resource ;
    rdfs:label "Item - I509 347  Offence related searches and seizures"@en-AU ;
    dct:isPartOf C2020A00012:507 ;
    dct:isReferencedBy C2020A00012: ;
    rdfs:comment "347  Offence related searches and seizures - Abrievated Graph Key: I509"@en-AU ;
    skos:definition "347  Offence related searches and seizures"@en-AU ;
    skos:narrower C2020A00012:507 ;
    skos:prefLabel "Item I509"@en-AU ;
    dcat:accessURL <https://www.legislation.gov.au/C2020A00012/2024-07-10/2024-07-10/text/original/epub/OEBPS/document_1/document_1.html#_Toc172119201> ;
    dcat:landingPage "https://www.legislation.gov.au/C2020A00012/2024-07-10/2024-07-10/text/original/epub/OEBPS/document_1/document_1.html#_Toc172119201"^^xsd:anyURI ;
    dcat:theme legcons:Item .

C2020A00012:51 a legcons:Item,
        owl:Class,
        dcat:Resource ;
    rdfs:label "Item - I51 37  Conveying or possessing goods that are intended to be exported to a temporarily prohibited place etc"@en-AU ;
    dct:isPartOf C2020A00012:28 ;
    dct:isReferencedBy C2020A00012: ;
    rdfs:comment "37  Conveying or possessing goods that are intended to be exported to a temporarily prohibited place etc - Abrievated Graph Key: I51"@en-AU ;
    skos:definition "37  Conveying or possessing goods that are intended to be exported to a temporarily prohibited place etc"@en-AU ;
    skos:narrower C2020A00012:28 ;
    skos:prefLabel "Item I51"@en-AU ;
    dcat:accessURL <https://www.legislation.gov.au/C2020A00012/2024-07-10/2024-07-10/text/original/epub/OEBPS/document_1/document_1.html#_Toc172118743> ;
    dcat:landingPage "https://www.legislation.gov.au/C2020A00012/2024-07-10/2024-07-10/text/original/epub/OEBPS/document_1/document_1.html#_Toc172118743"^^xsd:anyURI ;
    dcat:theme legcons:Item .

C2020A00012:511 a legcons:Item,
        owl:Class,
        dcat:Resource ;
    rdfs:label "Item - I511 348  Announcement before entry"@en-AU ;
    dct:isPartOf C2020A00012:510 ;
    dct:isReferencedBy C2020A00012: ;
    rdfs:comment "348  Announcement before entry - Abrievated Graph Key: I511"@en-AU ;
    skos:definition "348  Announcement before entry"@en-AU ;
    skos:narrower C2020A00012:510 ;
    skos:prefLabel "Item I511"@en-AU ;
    dcat:accessURL <https://www.legislation.gov.au/C2020A00012/2024-07-10/2024-07-10/text/original/epub/OEBPS/document_1/document_1.html#_Toc172119203> ;
    dcat:landingPage "https://www.legislation.gov.au/C2020A00012/2024-07-10/2024-07-10/text/original/epub/OEBPS/document_1/document_1.html#_Toc172119203"^^xsd:anyURI ;
    dcat:theme legcons:Item .

C2020A00012:512 a legcons:Item,
        owl:Class,
        dcat:Resource ;
    rdfs:label "Item - I512 349  Use of force in entering premises"@en-AU ;
    dct:isPartOf C2020A00012:510 ;
    dct:isReferencedBy C2020A00012: ;
    rdfs:comment "349  Use of force in entering premises - Abrievated Graph Key: I512"@en-AU ;
    skos:definition "349  Use of force in entering premises"@en-AU ;
    skos:narrower C2020A00012:510 ;
    skos:prefLabel "Item I512"@en-AU ;
    dcat:accessURL <https://www.legislation.gov.au/C2020A00012/2024-07-10/2024-07-10/text/original/epub/OEBPS/document_1/document_1.html#_Toc172119204> ;
    dcat:landingPage "https://www.legislation.gov.au/C2020A00012/2024-07-10/2024-07-10/text/original/epub/OEBPS/document_1/document_1.html#_Toc172119204"^^xsd:anyURI ;
    dcat:theme legcons:Item .

C2020A00012:514 a legcons:Item,
        owl:Class,
        dcat:Resource ;
    rdfs:label "Item - I514 350  Right to observe exercise of powers"@en-AU ;
    dct:isPartOf C2020A00012:513 ;
    dct:isReferencedBy C2020A00012: ;
    rdfs:comment "350  Right to observe exercise of powers - Abrievated Graph Key: I514"@en-AU ;
    skos:definition "350  Right to observe exercise of powers"@en-AU ;
    skos:narrower C2020A00012:513 ;
    skos:prefLabel "Item I514"@en-AU ;
    dcat:accessURL <https://www.legislation.gov.au/C2020A00012/2024-07-10/2024-07-10/text/original/epub/OEBPS/document_1/document_1.html#_Toc172119206> ;
    dcat:landingPage "https://www.legislation.gov.au/C2020A00012/2024-07-10/2024-07-10/text/original/epub/OEBPS/document_1/document_1.html#_Toc172119206"^^xsd:anyURI ;
    dcat:theme legcons:Item .

C2020A00012:515 a legcons:Item,
        owl:Class,
        dcat:Resource ;
    rdfs:label "Item - I515 351  Responsibility to provide facilities and assistance"@en-AU ;
    dct:isPartOf C2020A00012:513 ;
    dct:isReferencedBy C2020A00012: ;
    rdfs:comment "351  Responsibility to provide facilities and assistance - Abrievated Graph Key: I515"@en-AU ;
    skos:definition "351  Responsibility to provide facilities and assistance"@en-AU ;
    skos:narrower C2020A00012:513 ;
    skos:prefLabel "Item I515"@en-AU ;
    dcat:accessURL <https://www.legislation.gov.au/C2020A00012/2024-07-10/2024-07-10/text/original/epub/OEBPS/document_1/document_1.html#_Toc172119207> ;
    dcat:landingPage "https://www.legislation.gov.au/C2020A00012/2024-07-10/2024-07-10/text/original/epub/OEBPS/document_1/document_1.html#_Toc172119207"^^xsd:anyURI ;
    dcat:theme legcons:Item .

C2020A00012:518 a legcons:Item,
        owl:Class,
        dcat:Resource ;
    rdfs:label "Item - I518 352  Simplified outline of this Part"@en-AU ;
    dct:isPartOf C2020A00012:517 ;
    dct:isReferencedBy C2020A00012: ;
    rdfs:comment "352  Simplified outline of this Part - Abrievated Graph Key: I518"@en-AU ;
    skos:definition "352  Simplified outline of this Part"@en-AU ;
    skos:narrower C2020A00012:517 ;
    skos:prefLabel "Item I518"@en-AU ;
    dcat:accessURL <https://www.legislation.gov.au/C2020A00012/2024-07-10/2024-07-10/text/original/epub/OEBPS/document_1/document_1.html#_Toc172119210> ;
    dcat:landingPage "https://www.legislation.gov.au/C2020A00012/2024-07-10/2024-07-10/text/original/epub/OEBPS/document_1/document_1.html#_Toc172119210"^^xsd:anyURI ;
    dcat:theme legcons:Item .

C2020A00012:52 a legcons:Item,
        owl:Class,
        dcat:Resource ;
    rdfs:label "Item - I52 38  Exporting prescribed goodsnon compliance with prescribed export conditionsbasic contravention"@en-AU ;
    dct:isPartOf C2020A00012:28 ;
    dct:isReferencedBy C2020A00012: ;
    rdfs:comment "38  Exporting prescribed goodsnon compliance with prescribed export conditionsbasic contravention - Abrievated Graph Key: I52"@en-AU ;
    skos:definition "38  Exporting prescribed goodsnon compliance with prescribed export conditionsbasic contravention"@en-AU ;
    skos:narrower C2020A00012:28 ;
    skos:prefLabel "Item I52"@en-AU ;
    dcat:accessURL <https://www.legislation.gov.au/C2020A00012/2024-07-10/2024-07-10/text/original/epub/OEBPS/document_1/document_1.html#_Toc172118744> ;
    dcat:landingPage "https://www.legislation.gov.au/C2020A00012/2024-07-10/2024-07-10/text/original/epub/OEBPS/document_1/document_1.html#_Toc172118744"^^xsd:anyURI ;
    dcat:theme legcons:Item .

C2020A00012:520 a legcons:Item,
        owl:Class,
        dcat:Resource ;
    rdfs:label "Item - I520 353  Securing evidential material without consent or warrant in emergency situation"@en-AU ;
    dct:isPartOf C2020A00012:519 ;
    dct:isReferencedBy C2020A00012: ;
    rdfs:comment "353  Securing evidential material without consent or warrant in emergency situation - Abrievated Graph Key: I520"@en-AU ;
    skos:definition "353  Securing evidential material without consent or warrant in emergency situation"@en-AU ;
    skos:narrower C2020A00012:519 ;
    skos:prefLabel "Item I520"@en-AU ;
    dcat:accessURL <https://www.legislation.gov.au/C2020A00012/2024-07-10/2024-07-10/text/original/epub/OEBPS/document_1/document_1.html#_Toc172119212> ;
    dcat:landingPage "https://www.legislation.gov.au/C2020A00012/2024-07-10/2024-07-10/text/original/epub/OEBPS/document_1/document_1.html#_Toc172119212"^^xsd:anyURI ;
    dcat:theme legcons:Item .

C2020A00012:521 a legcons:Item,
        owl:Class,
        dcat:Resource ;
    rdfs:label "Item - I521 354  Stopping and searching conveyance without warrant in emergency situation"@en-AU ;
    dct:isPartOf C2020A00012:519 ;
    dct:isReferencedBy C2020A00012: ;
    rdfs:comment "354  Stopping and searching conveyance without warrant in emergency situation - Abrievated Graph Key: I521"@en-AU ;
    skos:definition "354  Stopping and searching conveyance without warrant in emergency situation"@en-AU ;
    skos:narrower C2020A00012:519 ;
    skos:prefLabel "Item I521"@en-AU ;
    dcat:accessURL <https://www.legislation.gov.au/C2020A00012/2024-07-10/2024-07-10/text/original/epub/OEBPS/document_1/document_1.html#_Toc172119213> ;
    dcat:landingPage "https://www.legislation.gov.au/C2020A00012/2024-07-10/2024-07-10/text/original/epub/OEBPS/document_1/document_1.html#_Toc172119213"^^xsd:anyURI ;
    dcat:theme legcons:Item .

C2020A00012:524 a legcons:Item,
        owl:Class,
        dcat:Resource ;
    rdfs:label "Item - I524 355  Simplified outline of this Part"@en-AU ;
    dct:isPartOf C2020A00012:523 ;
    dct:isReferencedBy C2020A00012: ;
    rdfs:comment "355  Simplified outline of this Part - Abrievated Graph Key: I524"@en-AU ;
    skos:definition "355  Simplified outline of this Part"@en-AU ;
    skos:narrower C2020A00012:523 ;
    skos:prefLabel "Item I524"@en-AU ;
    dcat:accessURL <https://www.legislation.gov.au/C2020A00012/2024-07-10/2024-07-10/text/original/epub/OEBPS/document_1/document_1.html#_Toc172119216> ;
    dcat:landingPage "https://www.legislation.gov.au/C2020A00012/2024-07-10/2024-07-10/text/original/epub/OEBPS/document_1/document_1.html#_Toc172119216"^^xsd:anyURI ;
    dcat:theme legcons:Item .

C2020A00012:526 a legcons:Item,
        owl:Class,
        dcat:Resource ;
    rdfs:label "Item - I526 356  Basic operation of civil penalties under Part 4 of the Regulatory Powers Act"@en-AU ;
    dct:isPartOf C2020A00012:525 ;
    dct:isReferencedBy C2020A00012: ;
    rdfs:comment "356  Basic operation of civil penalties under Part 4 of the Regulatory Powers Act - Abrievated Graph Key: I526"@en-AU ;
    skos:definition "356  Basic operation of civil penalties under Part 4 of the Regulatory Powers Act"@en-AU ;
    skos:narrower C2020A00012:525 ;
    skos:prefLabel "Item I526"@en-AU ;
    dcat:accessURL <https://www.legislation.gov.au/C2020A00012/2024-07-10/2024-07-10/text/original/epub/OEBPS/document_1/document_1.html#_Toc172119218> ;
    dcat:landingPage "https://www.legislation.gov.au/C2020A00012/2024-07-10/2024-07-10/text/original/epub/OEBPS/document_1/document_1.html#_Toc172119218"^^xsd:anyURI ;
    dcat:theme legcons:Item .

C2020A00012:529 a legcons:Item,
        owl:Class,
        dcat:Resource ;
    rdfs:label "Item - I529 358  Simplified outline of this Part"@en-AU ;
    dct:isPartOf C2020A00012:528 ;
    dct:isReferencedBy C2020A00012: ;
    rdfs:comment "358  Simplified outline of this Part - Abrievated Graph Key: I529"@en-AU ;
    skos:definition "358  Simplified outline of this Part"@en-AU ;
    skos:narrower C2020A00012:528 ;
    skos:prefLabel "Item I529"@en-AU ;
    dcat:accessURL <https://www.legislation.gov.au/C2020A00012/2024-07-10/2024-07-10/text/original/epub/OEBPS/document_1/document_1.html#_Toc172119221> ;
    dcat:landingPage "https://www.legislation.gov.au/C2020A00012/2024-07-10/2024-07-10/text/original/epub/OEBPS/document_1/document_1.html#_Toc172119221"^^xsd:anyURI ;
    dcat:theme legcons:Item .

C2020A00012:53 a legcons:Item,
        owl:Class,
        dcat:Resource ;
    rdfs:label "Item - I53 39  Exporting prescribed goodsnon compliance with prescribed export conditionsintention to obtain commercial advantage"@en-AU ;
    dct:isPartOf C2020A00012:28 ;
    dct:isReferencedBy C2020A00012: ;
    rdfs:comment "39  Exporting prescribed goodsnon compliance with prescribed export conditionsintention to obtain commercial advantage - Abrievated Graph Key: I53"@en-AU ;
    skos:definition "39  Exporting prescribed goodsnon compliance with prescribed export conditionsintention to obtain commercial advantage"@en-AU ;
    skos:narrower C2020A00012:28 ;
    skos:prefLabel "Item I53"@en-AU ;
    dcat:accessURL <https://www.legislation.gov.au/C2020A00012/2024-07-10/2024-07-10/text/original/epub/OEBPS/document_1/document_1.html#_Toc172118745> ;
    dcat:landingPage "https://www.legislation.gov.au/C2020A00012/2024-07-10/2024-07-10/text/original/epub/OEBPS/document_1/document_1.html#_Toc172118745"^^xsd:anyURI ;
    dcat:theme legcons:Item .

C2020A00012:531 a legcons:Item,
        owl:Class,
        dcat:Resource ;
    rdfs:label "Item - I531 359  Basic provisions for infringement notices under Part 5 of the Regulatory Powers Act"@en-AU ;
    dct:isPartOf C2020A00012:530 ;
    dct:isReferencedBy C2020A00012: ;
    rdfs:comment "359  Basic provisions for infringement notices under Part 5 of the Regulatory Powers Act - Abrievated Graph Key: I531"@en-AU ;
    skos:definition "359  Basic provisions for infringement notices under Part 5 of the Regulatory Powers Act"@en-AU ;
    skos:narrower C2020A00012:530 ;
    skos:prefLabel "Item I531"@en-AU ;
    dcat:accessURL <https://www.legislation.gov.au/C2020A00012/2024-07-10/2024-07-10/text/original/epub/OEBPS/document_1/document_1.html#_Toc172119223> ;
    dcat:landingPage "https://www.legislation.gov.au/C2020A00012/2024-07-10/2024-07-10/text/original/epub/OEBPS/document_1/document_1.html#_Toc172119223"^^xsd:anyURI ;
    dcat:theme legcons:Item .

C2020A00012:532 a legcons:Item,
        owl:Class,
        dcat:Resource ;
    rdfs:label "Item - I532 360  Modifications of Part 5 of the Regulatory Powers Act"@en-AU ;
    dct:isPartOf C2020A00012:530 ;
    dct:isReferencedBy C2020A00012: ;
    rdfs:comment "360  Modifications of Part 5 of the Regulatory Powers Act - Abrievated Graph Key: I532"@en-AU ;
    skos:definition "360  Modifications of Part 5 of the Regulatory Powers Act"@en-AU ;
    skos:narrower C2020A00012:530 ;
    skos:prefLabel "Item I532"@en-AU ;
    dcat:accessURL <https://www.legislation.gov.au/C2020A00012/2024-07-10/2024-07-10/text/original/epub/OEBPS/document_1/document_1.html#_Toc172119224> ;
    dcat:landingPage "https://www.legislation.gov.au/C2020A00012/2024-07-10/2024-07-10/text/original/epub/OEBPS/document_1/document_1.html#_Toc172119224"^^xsd:anyURI ;
    dcat:theme legcons:Item .

C2020A00012:535 a legcons:Item,
        owl:Class,
        dcat:Resource ;
    rdfs:label "Item - I535 361  Simplified outline of this Part"@en-AU ;
    dct:isPartOf C2020A00012:534 ;
    dct:isReferencedBy C2020A00012: ;
    rdfs:comment "361  Simplified outline of this Part - Abrievated Graph Key: I535"@en-AU ;
    skos:definition "361  Simplified outline of this Part"@en-AU ;
    skos:narrower C2020A00012:534 ;
    skos:prefLabel "Item I535"@en-AU ;
    dcat:accessURL <https://www.legislation.gov.au/C2020A00012/2024-07-10/2024-07-10/text/original/epub/OEBPS/document_1/document_1.html#_Toc172119227> ;
    dcat:landingPage "https://www.legislation.gov.au/C2020A00012/2024-07-10/2024-07-10/text/original/epub/OEBPS/document_1/document_1.html#_Toc172119227"^^xsd:anyURI ;
    dcat:theme legcons:Item .

C2020A00012:537 a legcons:Item,
        owl:Class,
        dcat:Resource ;
    rdfs:label "Item - I537 362  Enforceable undertakings"@en-AU ;
    dct:isPartOf C2020A00012:536 ;
    dct:isReferencedBy C2020A00012: ;
    rdfs:comment "362  Enforceable undertakings - Abrievated Graph Key: I537"@en-AU ;
    skos:definition "362  Enforceable undertakings"@en-AU ;
    skos:narrower C2020A00012:536 ;
    skos:prefLabel "Item I537"@en-AU ;
    dcat:accessURL <https://www.legislation.gov.au/C2020A00012/2024-07-10/2024-07-10/text/original/epub/OEBPS/document_1/document_1.html#_Toc172119229> ;
    dcat:landingPage "https://www.legislation.gov.au/C2020A00012/2024-07-10/2024-07-10/text/original/epub/OEBPS/document_1/document_1.html#_Toc172119229"^^xsd:anyURI ;
    dcat:theme legcons:Item .

C2020A00012:54 a legcons:Item,
        owl:Class,
        dcat:Resource ;
    rdfs:label "Item - I54 40  Exporting prescribed goodsnon compliance with prescribed export conditionseconomic consequences for Australia"@en-AU ;
    dct:isPartOf C2020A00012:28 ;
    dct:isReferencedBy C2020A00012: ;
    rdfs:comment "40  Exporting prescribed goodsnon compliance with prescribed export conditionseconomic consequences for Australia - Abrievated Graph Key: I54"@en-AU ;
    skos:definition "40  Exporting prescribed goodsnon compliance with prescribed export conditionseconomic consequences for Australia"@en-AU ;
    skos:narrower C2020A00012:28 ;
    skos:prefLabel "Item I54"@en-AU ;
    dcat:accessURL <https://www.legislation.gov.au/C2020A00012/2024-07-10/2024-07-10/text/original/epub/OEBPS/document_1/document_1.html#_Toc172118746> ;
    dcat:landingPage "https://www.legislation.gov.au/C2020A00012/2024-07-10/2024-07-10/text/original/epub/OEBPS/document_1/document_1.html#_Toc172118746"^^xsd:anyURI ;
    dcat:theme legcons:Item .

C2020A00012:540 a legcons:Item,
        owl:Class,
        dcat:Resource ;
    rdfs:label "Item - I540 363  Simplified outline of this Part"@en-AU ;
    dct:isPartOf C2020A00012:539 ;
    dct:isReferencedBy C2020A00012: ;
    rdfs:comment "363  Simplified outline of this Part - Abrievated Graph Key: I540"@en-AU ;
    skos:definition "363  Simplified outline of this Part"@en-AU ;
    skos:narrower C2020A00012:539 ;
    skos:prefLabel "Item I540"@en-AU ;
    dcat:accessURL <https://www.legislation.gov.au/C2020A00012/2024-07-10/2024-07-10/text/original/epub/OEBPS/document_1/document_1.html#_Toc172119232> ;
    dcat:landingPage "https://www.legislation.gov.au/C2020A00012/2024-07-10/2024-07-10/text/original/epub/OEBPS/document_1/document_1.html#_Toc172119232"^^xsd:anyURI ;
    dcat:theme legcons:Item .

C2020A00012:542 a legcons:Item,
        owl:Class,
        dcat:Resource ;
    rdfs:label "Item - I542 364  Injunctions"@en-AU ;
    dct:isPartOf C2020A00012:541 ;
    dct:isReferencedBy C2020A00012: ;
    rdfs:comment "364  Injunctions - Abrievated Graph Key: I542"@en-AU ;
    skos:definition "364  Injunctions"@en-AU ;
    skos:narrower C2020A00012:541 ;
    skos:prefLabel "Item I542"@en-AU ;
    dcat:accessURL <https://www.legislation.gov.au/C2020A00012/2024-07-10/2024-07-10/text/original/epub/OEBPS/document_1/document_1.html#_Toc172119234> ;
    dcat:landingPage "https://www.legislation.gov.au/C2020A00012/2024-07-10/2024-07-10/text/original/epub/OEBPS/document_1/document_1.html#_Toc172119234"^^xsd:anyURI ;
    dcat:theme legcons:Item .

C2020A00012:544 a legcons:Item,
        owl:Class,
        dcat:Resource ;
    rdfs:label "Item - I544 364 A  Simplified outline of this Part"@en-AU ;
    dct:isPartOf C2020A00012:543 ;
    dct:isReferencedBy C2020A00012: ;
    rdfs:comment "364 A  Simplified outline of this Part - Abrievated Graph Key: I544"@en-AU ;
    skos:definition "364 A  Simplified outline of this Part"@en-AU ;
    skos:narrower C2020A00012:543 ;
    skos:prefLabel "Item I544"@en-AU ;
    dcat:accessURL <https://www.legislation.gov.au/C2020A00012/2024-07-10/2024-07-10/text/original/epub/OEBPS/document_1/document_1.html#_Toc172119236> ;
    dcat:landingPage "https://www.legislation.gov.au/C2020A00012/2024-07-10/2024-07-10/text/original/epub/OEBPS/document_1/document_1.html#_Toc172119236"^^xsd:anyURI ;
    dcat:theme legcons:Item .

C2020A00012:545 a legcons:Item,
        owl:Class,
        dcat:Resource ;
    rdfs:label "Item - I545 364 B  Criminal liability for executive officers of bodies corporate"@en-AU ;
    dct:isPartOf C2020A00012:543 ;
    dct:isReferencedBy C2020A00012: ;
    rdfs:comment "364 B  Criminal liability for executive officers of bodies corporate - Abrievated Graph Key: I545"@en-AU ;
    skos:definition "364 B  Criminal liability for executive officers of bodies corporate"@en-AU ;
    skos:narrower C2020A00012:543 ;
    skos:prefLabel "Item I545"@en-AU ;
    dcat:accessURL <https://www.legislation.gov.au/C2020A00012/2024-07-10/2024-07-10/text/original/epub/OEBPS/document_1/document_1.html#_Toc172119237> ;
    dcat:landingPage "https://www.legislation.gov.au/C2020A00012/2024-07-10/2024-07-10/text/original/epub/OEBPS/document_1/document_1.html#_Toc172119237"^^xsd:anyURI ;
    dcat:theme legcons:Item .

C2020A00012:546 a legcons:Item,
        owl:Class,
        dcat:Resource ;
    rdfs:label "Item - I546 364 C  Civil liability for executive officers of bodies corporate"@en-AU ;
    dct:isPartOf C2020A00012:543 ;
    dct:isReferencedBy C2020A00012: ;
    rdfs:comment "364 C  Civil liability for executive officers of bodies corporate - Abrievated Graph Key: I546"@en-AU ;
    skos:definition "364 C  Civil liability for executive officers of bodies corporate"@en-AU ;
    skos:narrower C2020A00012:543 ;
    skos:prefLabel "Item I546"@en-AU ;
    dcat:accessURL <https://www.legislation.gov.au/C2020A00012/2024-07-10/2024-07-10/text/original/epub/OEBPS/document_1/document_1.html#_Toc172119238> ;
    dcat:landingPage "https://www.legislation.gov.au/C2020A00012/2024-07-10/2024-07-10/text/original/epub/OEBPS/document_1/document_1.html#_Toc172119238"^^xsd:anyURI ;
    dcat:theme legcons:Item .

C2020A00012:547 a legcons:Item,
        owl:Class,
        dcat:Resource ;
    rdfs:label "Item - I547 364 D  Civil penaltyindemnification of executive officers"@en-AU ;
    dct:isPartOf C2020A00012:543 ;
    dct:isReferencedBy C2020A00012: ;
    rdfs:comment "364 D  Civil penaltyindemnification of executive officers - Abrievated Graph Key: I547"@en-AU ;
    skos:definition "364 D  Civil penaltyindemnification of executive officers"@en-AU ;
    skos:narrower C2020A00012:543 ;
    skos:prefLabel "Item I547"@en-AU ;
    dcat:accessURL <https://www.legislation.gov.au/C2020A00012/2024-07-10/2024-07-10/text/original/epub/OEBPS/document_1/document_1.html#_Toc172119239> ;
    dcat:landingPage "https://www.legislation.gov.au/C2020A00012/2024-07-10/2024-07-10/text/original/epub/OEBPS/document_1/document_1.html#_Toc172119239"^^xsd:anyURI ;
    dcat:theme legcons:Item .

C2020A00012:548 a legcons:Item,
        owl:Class,
        dcat:Resource ;
    rdfs:label "Item - I548 364 E  Certain indemnities not authorised and certain documents void"@en-AU ;
    dct:isPartOf C2020A00012:543 ;
    dct:isReferencedBy C2020A00012: ;
    rdfs:comment "364 E  Certain indemnities not authorised and certain documents void - Abrievated Graph Key: I548"@en-AU ;
    skos:definition "364 E  Certain indemnities not authorised and certain documents void"@en-AU ;
    skos:narrower C2020A00012:543 ;
    skos:prefLabel "Item I548"@en-AU ;
    dcat:accessURL <https://www.legislation.gov.au/C2020A00012/2024-07-10/2024-07-10/text/original/epub/OEBPS/document_1/document_1.html#_Toc172119240> ;
    dcat:landingPage "https://www.legislation.gov.au/C2020A00012/2024-07-10/2024-07-10/text/original/epub/OEBPS/document_1/document_1.html#_Toc172119240"^^xsd:anyURI ;
    dcat:theme legcons:Item .

C2020A00012:549 a legcons:Item,
        owl:Class,
        dcat:Resource ;
    rdfs:label "Item - I549 364 F  Adverse publicity orders"@en-AU ;
    dct:isPartOf C2020A00012:543 ;
    dct:isReferencedBy C2020A00012: ;
    rdfs:comment "364 F  Adverse publicity orders - Abrievated Graph Key: I549"@en-AU ;
    skos:definition "364 F  Adverse publicity orders"@en-AU ;
    skos:narrower C2020A00012:543 ;
    skos:prefLabel "Item I549"@en-AU ;
    dcat:accessURL <https://www.legislation.gov.au/C2020A00012/2024-07-10/2024-07-10/text/original/epub/OEBPS/document_1/document_1.html#_Toc172119241> ;
    dcat:landingPage "https://www.legislation.gov.au/C2020A00012/2024-07-10/2024-07-10/text/original/epub/OEBPS/document_1/document_1.html#_Toc172119241"^^xsd:anyURI ;
    dcat:theme legcons:Item .

C2020A00012:55 a legcons:Item,
        owl:Class,
        dcat:Resource ;
    rdfs:label "Item - I55 41  Conveying or possessing prescribed goods that are intended to be exported in contravention of conditions etc"@en-AU ;
    dct:isPartOf C2020A00012:28 ;
    dct:isReferencedBy C2020A00012: ;
    rdfs:comment "41  Conveying or possessing prescribed goods that are intended to be exported in contravention of conditions etc - Abrievated Graph Key: I55"@en-AU ;
    skos:definition "41  Conveying or possessing prescribed goods that are intended to be exported in contravention of conditions etc"@en-AU ;
    skos:narrower C2020A00012:28 ;
    skos:prefLabel "Item I55"@en-AU ;
    dcat:accessURL <https://www.legislation.gov.au/C2020A00012/2024-07-10/2024-07-10/text/original/epub/OEBPS/document_1/document_1.html#_Toc172118747> ;
    dcat:landingPage "https://www.legislation.gov.au/C2020A00012/2024-07-10/2024-07-10/text/original/epub/OEBPS/document_1/document_1.html#_Toc172118747"^^xsd:anyURI ;
    dcat:theme legcons:Item .

C2020A00012:552 a legcons:Item,
        owl:Class,
        dcat:Resource ;
    rdfs:label "Item - I552 365  Simplified outline of this Part"@en-AU ;
    dct:isPartOf C2020A00012:551 ;
    dct:isReferencedBy C2020A00012: ;
    rdfs:comment "365  Simplified outline of this Part - Abrievated Graph Key: I552"@en-AU ;
    skos:definition "365  Simplified outline of this Part"@en-AU ;
    skos:narrower C2020A00012:551 ;
    skos:prefLabel "Item I552"@en-AU ;
    dcat:accessURL <https://www.legislation.gov.au/C2020A00012/2024-07-10/2024-07-10/text/original/epub/OEBPS/document_1/document_1.html#_Toc172119244> ;
    dcat:landingPage "https://www.legislation.gov.au/C2020A00012/2024-07-10/2024-07-10/text/original/epub/OEBPS/document_1/document_1.html#_Toc172119244"^^xsd:anyURI ;
    dcat:theme legcons:Item .

C2020A00012:554 a legcons:Item,
        owl:Class,
        dcat:Resource ;
    rdfs:label "Item - I554 366  Persons assisting authorised officers"@en-AU ;
    dct:isPartOf C2020A00012:553 ;
    dct:isReferencedBy C2020A00012: ;
    rdfs:comment "366  Persons assisting authorised officers - Abrievated Graph Key: I554"@en-AU ;
    skos:definition "366  Persons assisting authorised officers"@en-AU ;
    skos:narrower C2020A00012:553 ;
    skos:prefLabel "Item I554"@en-AU ;
    dcat:accessURL <https://www.legislation.gov.au/C2020A00012/2024-07-10/2024-07-10/text/original/epub/OEBPS/document_1/document_1.html#_Toc172119246> ;
    dcat:landingPage "https://www.legislation.gov.au/C2020A00012/2024-07-10/2024-07-10/text/original/epub/OEBPS/document_1/document_1.html#_Toc172119246"^^xsd:anyURI ;
    dcat:theme legcons:Item .

C2020A00012:556 a legcons:Item,
        owl:Class,
        dcat:Resource ;
    rdfs:label "Item - I556 367  Civil penalty provision for false or misleading statements in applications"@en-AU ;
    dct:isPartOf C2020A00012:555 ;
    dct:isReferencedBy C2020A00012: ;
    rdfs:comment "367  Civil penalty provision for false or misleading statements in applications - Abrievated Graph Key: I556"@en-AU ;
    skos:definition "367  Civil penalty provision for false or misleading statements in applications"@en-AU ;
    skos:narrower C2020A00012:555 ;
    skos:prefLabel "Item I556"@en-AU ;
    dcat:accessURL <https://www.legislation.gov.au/C2020A00012/2024-07-10/2024-07-10/text/original/epub/OEBPS/document_1/document_1.html#_Toc172119248> ;
    dcat:landingPage "https://www.legislation.gov.au/C2020A00012/2024-07-10/2024-07-10/text/original/epub/OEBPS/document_1/document_1.html#_Toc172119248"^^xsd:anyURI ;
    dcat:theme legcons:Item .

C2020A00012:557 a legcons:Item,
        owl:Class,
        dcat:Resource ;
    rdfs:label "Item - I557 368  Civil penalty provision for false or misleading information"@en-AU ;
    dct:isPartOf C2020A00012:555 ;
    dct:isReferencedBy C2020A00012: ;
    rdfs:comment "368  Civil penalty provision for false or misleading information - Abrievated Graph Key: I557"@en-AU ;
    skos:definition "368  Civil penalty provision for false or misleading information"@en-AU ;
    skos:narrower C2020A00012:555 ;
    skos:prefLabel "Item I557"@en-AU ;
    dcat:accessURL <https://www.legislation.gov.au/C2020A00012/2024-07-10/2024-07-10/text/original/epub/OEBPS/document_1/document_1.html#_Toc172119249> ;
    dcat:landingPage "https://www.legislation.gov.au/C2020A00012/2024-07-10/2024-07-10/text/original/epub/OEBPS/document_1/document_1.html#_Toc172119249"^^xsd:anyURI ;
    dcat:theme legcons:Item .

C2020A00012:558 a legcons:Item,
        owl:Class,
        dcat:Resource ;
    rdfs:label "Item - I558 369  Civil penalty provision for false or misleading documents"@en-AU ;
    dct:isPartOf C2020A00012:555 ;
    dct:isReferencedBy C2020A00012: ;
    rdfs:comment "369  Civil penalty provision for false or misleading documents - Abrievated Graph Key: I558"@en-AU ;
    skos:definition "369  Civil penalty provision for false or misleading documents"@en-AU ;
    skos:narrower C2020A00012:555 ;
    skos:prefLabel "Item I558"@en-AU ;
    dcat:accessURL <https://www.legislation.gov.au/C2020A00012/2024-07-10/2024-07-10/text/original/epub/OEBPS/document_1/document_1.html#_Toc172119250> ;
    dcat:landingPage "https://www.legislation.gov.au/C2020A00012/2024-07-10/2024-07-10/text/original/epub/OEBPS/document_1/document_1.html#_Toc172119250"^^xsd:anyURI ;
    dcat:theme legcons:Item .

C2020A00012:56 a legcons:Item,
        owl:Class,
        dcat:Resource ;
    rdfs:label "Item - I56 42  Exporting prescribed goods to a particular placenon compliance with prescribed export conditionsbasic contravention"@en-AU ;
    dct:isPartOf C2020A00012:28 ;
    dct:isReferencedBy C2020A00012: ;
    rdfs:comment "42  Exporting prescribed goods to a particular placenon compliance with prescribed export conditionsbasic contravention - Abrievated Graph Key: I56"@en-AU ;
    skos:definition "42  Exporting prescribed goods to a particular placenon compliance with prescribed export conditionsbasic contravention"@en-AU ;
    skos:narrower C2020A00012:28 ;
    skos:prefLabel "Item I56"@en-AU ;
    dcat:accessURL <https://www.legislation.gov.au/C2020A00012/2024-07-10/2024-07-10/text/original/epub/OEBPS/document_1/document_1.html#_Toc172118748> ;
    dcat:landingPage "https://www.legislation.gov.au/C2020A00012/2024-07-10/2024-07-10/text/original/epub/OEBPS/document_1/document_1.html#_Toc172118748"^^xsd:anyURI ;
    dcat:theme legcons:Item .

C2020A00012:560 a legcons:Item,
        owl:Class,
        dcat:Resource ;
    rdfs:label "Item - I560 370  Physical elements of offences"@en-AU ;
    dct:isPartOf C2020A00012:559 ;
    dct:isReferencedBy C2020A00012: ;
    rdfs:comment "370  Physical elements of offences - Abrievated Graph Key: I560"@en-AU ;
    skos:definition "370  Physical elements of offences"@en-AU ;
    skos:narrower C2020A00012:559 ;
    skos:prefLabel "Item I560"@en-AU ;
    dcat:accessURL <https://www.legislation.gov.au/C2020A00012/2024-07-10/2024-07-10/text/original/epub/OEBPS/document_1/document_1.html#_Toc172119252> ;
    dcat:landingPage "https://www.legislation.gov.au/C2020A00012/2024-07-10/2024-07-10/text/original/epub/OEBPS/document_1/document_1.html#_Toc172119252"^^xsd:anyURI ;
    dcat:theme legcons:Item .

C2020A00012:561 a legcons:Item,
        owl:Class,
        dcat:Resource ;
    rdfs:label "Item - I561 371  Contravening an offence provision or a civil penalty provision"@en-AU ;
    dct:isPartOf C2020A00012:559 ;
    dct:isReferencedBy C2020A00012: ;
    rdfs:comment "371  Contravening an offence provision or a civil penalty provision - Abrievated Graph Key: I561"@en-AU ;
    skos:definition "371  Contravening an offence provision or a civil penalty provision"@en-AU ;
    skos:narrower C2020A00012:559 ;
    skos:prefLabel "Item I561"@en-AU ;
    dcat:accessURL <https://www.legislation.gov.au/C2020A00012/2024-07-10/2024-07-10/text/original/epub/OEBPS/document_1/document_1.html#_Toc172119253> ;
    dcat:landingPage "https://www.legislation.gov.au/C2020A00012/2024-07-10/2024-07-10/text/original/epub/OEBPS/document_1/document_1.html#_Toc172119253"^^xsd:anyURI ;
    dcat:theme legcons:Item .

C2020A00012:563 a legcons:Item,
        owl:Class,
        dcat:Resource ;
    rdfs:label "Item - I563 372  Fit and proper person test"@en-AU ;
    dct:isPartOf C2020A00012:562 ;
    dct:isReferencedBy C2020A00012: ;
    rdfs:comment "372  Fit and proper person test - Abrievated Graph Key: I563"@en-AU ;
    skos:definition "372  Fit and proper person test"@en-AU ;
    skos:narrower C2020A00012:562 ;
    skos:prefLabel "Item I563"@en-AU ;
    dcat:accessURL <https://www.legislation.gov.au/C2020A00012/2024-07-10/2024-07-10/text/original/epub/OEBPS/document_1/document_1.html#_Toc172119255> ;
    dcat:landingPage "https://www.legislation.gov.au/C2020A00012/2024-07-10/2024-07-10/text/original/epub/OEBPS/document_1/document_1.html#_Toc172119255"^^xsd:anyURI ;
    dcat:theme legcons:Item .

C2020A00012:564 a legcons:Item,
        owl:Class,
        dcat:Resource ;
    rdfs:label "Item - I564 373  Rules may prescribe kinds of persons that are required to be fit and proper persons for the purposes of Chapter 5 or 6"@en-AU ;
    dct:isPartOf C2020A00012:562 ;
    dct:isReferencedBy C2020A00012: ;
    rdfs:comment "373  Rules may prescribe kinds of persons that are required to be fit and proper persons for the purposes of Chapter 5 or 6 - Abrievated Graph Key: I564"@en-AU ;
    skos:definition "373  Rules may prescribe kinds of persons that are required to be fit and proper persons for the purposes of Chapter 5 or 6"@en-AU ;
    skos:narrower C2020A00012:562 ;
    skos:prefLabel "Item I564"@en-AU ;
    dcat:accessURL <https://www.legislation.gov.au/C2020A00012/2024-07-10/2024-07-10/text/original/epub/OEBPS/document_1/document_1.html#_Toc172119256> ;
    dcat:landingPage "https://www.legislation.gov.au/C2020A00012/2024-07-10/2024-07-10/text/original/epub/OEBPS/document_1/document_1.html#_Toc172119256"^^xsd:anyURI ;
    dcat:theme legcons:Item .

C2020A00012:565 a legcons:Item,
        owl:Class,
        dcat:Resource ;
    rdfs:label "Item - I565 374  Notification of conviction of offence or order to pay pecuniary penalty"@en-AU ;
    dct:isPartOf C2020A00012:562 ;
    dct:isReferencedBy C2020A00012: ;
    rdfs:comment "374  Notification of conviction of offence or order to pay pecuniary penalty - Abrievated Graph Key: I565"@en-AU ;
    skos:definition "374  Notification of conviction of offence or order to pay pecuniary penalty"@en-AU ;
    skos:narrower C2020A00012:562 ;
    skos:prefLabel "Item I565"@en-AU ;
    dcat:accessURL <https://www.legislation.gov.au/C2020A00012/2024-07-10/2024-07-10/text/original/epub/OEBPS/document_1/document_1.html#_Toc172119257> ;
    dcat:landingPage "https://www.legislation.gov.au/C2020A00012/2024-07-10/2024-07-10/text/original/epub/OEBPS/document_1/document_1.html#_Toc172119257"^^xsd:anyURI ;
    dcat:theme legcons:Item .

C2020A00012:569 a legcons:Item,
        owl:Class,
        dcat:Resource ;
    rdfs:label "Item - I569 375  Simplified outline of this Part"@en-AU ;
    dct:isPartOf C2020A00012:568 ;
    dct:isReferencedBy C2020A00012: ;
    rdfs:comment "375  Simplified outline of this Part - Abrievated Graph Key: I569"@en-AU ;
    skos:definition "375  Simplified outline of this Part"@en-AU ;
    skos:narrower C2020A00012:568 ;
    skos:prefLabel "Item I569"@en-AU ;
    dcat:accessURL <https://www.legislation.gov.au/C2020A00012/2024-07-10/2024-07-10/text/original/epub/OEBPS/document_1/document_1.html#_Toc172119261> ;
    dcat:landingPage "https://www.legislation.gov.au/C2020A00012/2024-07-10/2024-07-10/text/original/epub/OEBPS/document_1/document_1.html#_Toc172119261"^^xsd:anyURI ;
    dcat:theme legcons:Item .

C2020A00012:57 a legcons:Item,
        owl:Class,
        dcat:Resource ;
    rdfs:label "Item - I57 43  Exporting prescribed goods to a particular placenon compliance with prescribed export conditionsintention to obtain commercial advantage"@en-AU ;
    dct:isPartOf C2020A00012:28 ;
    dct:isReferencedBy C2020A00012: ;
    rdfs:comment "43  Exporting prescribed goods to a particular placenon compliance with prescribed export conditionsintention to obtain commercial advantage - Abrievated Graph Key: I57"@en-AU ;
    skos:definition "43  Exporting prescribed goods to a particular placenon compliance with prescribed export conditionsintention to obtain commercial advantage"@en-AU ;
    skos:narrower C2020A00012:28 ;
    skos:prefLabel "Item I57"@en-AU ;
    dcat:accessURL <https://www.legislation.gov.au/C2020A00012/2024-07-10/2024-07-10/text/original/epub/OEBPS/document_1/document_1.html#_Toc172118749> ;
    dcat:landingPage "https://www.legislation.gov.au/C2020A00012/2024-07-10/2024-07-10/text/original/epub/OEBPS/document_1/document_1.html#_Toc172118749"^^xsd:anyURI ;
    dcat:theme legcons:Item .

C2020A00012:571 a legcons:Item,
        owl:Class,
        dcat:Resource ;
    rdfs:label "Item - I571 376  Applications to which this Division applies"@en-AU ;
    dct:isPartOf C2020A00012:570 ;
    dct:isReferencedBy C2020A00012: ;
    rdfs:comment "376  Applications to which this Division applies - Abrievated Graph Key: I571"@en-AU ;
    skos:definition "376  Applications to which this Division applies"@en-AU ;
    skos:narrower C2020A00012:570 ;
    skos:prefLabel "Item I571"@en-AU ;
    dcat:accessURL <https://www.legislation.gov.au/C2020A00012/2024-07-10/2024-07-10/text/original/epub/OEBPS/document_1/document_1.html#_Toc172119263> ;
    dcat:landingPage "https://www.legislation.gov.au/C2020A00012/2024-07-10/2024-07-10/text/original/epub/OEBPS/document_1/document_1.html#_Toc172119263"^^xsd:anyURI ;
    dcat:theme legcons:Item .

C2020A00012:572 a legcons:Item,
        owl:Class,
        dcat:Resource ;
    rdfs:label "Item - I572 377  Requirements for applications"@en-AU ;
    dct:isPartOf C2020A00012:570 ;
    dct:isReferencedBy C2020A00012: ;
    rdfs:comment "377  Requirements for applications - Abrievated Graph Key: I572"@en-AU ;
    skos:definition "377  Requirements for applications"@en-AU ;
    skos:narrower C2020A00012:570 ;
    skos:prefLabel "Item I572"@en-AU ;
    dcat:accessURL <https://www.legislation.gov.au/C2020A00012/2024-07-10/2024-07-10/text/original/epub/OEBPS/document_1/document_1.html#_Toc172119264> ;
    dcat:landingPage "https://www.legislation.gov.au/C2020A00012/2024-07-10/2024-07-10/text/original/epub/OEBPS/document_1/document_1.html#_Toc172119264"^^xsd:anyURI ;
    dcat:theme legcons:Item .

C2020A00012:573 a legcons:Item,
        owl:Class,
        dcat:Resource ;
    rdfs:label "Item - I573 378  Additional or corrected information"@en-AU ;
    dct:isPartOf C2020A00012:570 ;
    dct:isReferencedBy C2020A00012: ;
    rdfs:comment "378  Additional or corrected information - Abrievated Graph Key: I573"@en-AU ;
    skos:definition "378  Additional or corrected information"@en-AU ;
    skos:narrower C2020A00012:570 ;
    skos:prefLabel "Item I573"@en-AU ;
    dcat:accessURL <https://www.legislation.gov.au/C2020A00012/2024-07-10/2024-07-10/text/original/epub/OEBPS/document_1/document_1.html#_Toc172119265> ;
    dcat:landingPage "https://www.legislation.gov.au/C2020A00012/2024-07-10/2024-07-10/text/original/epub/OEBPS/document_1/document_1.html#_Toc172119265"^^xsd:anyURI ;
    dcat:theme legcons:Item .

C2020A00012:574 a legcons:Item,
        owl:Class,
        dcat:Resource ;
    rdfs:label "Item - I574 379  Dealing with applications"@en-AU ;
    dct:isPartOf C2020A00012:570 ;
    dct:isReferencedBy C2020A00012: ;
    rdfs:comment "379  Dealing with applications - Abrievated Graph Key: I574"@en-AU ;
    skos:definition "379  Dealing with applications"@en-AU ;
    skos:narrower C2020A00012:570 ;
    skos:prefLabel "Item I574"@en-AU ;
    dcat:accessURL <https://www.legislation.gov.au/C2020A00012/2024-07-10/2024-07-10/text/original/epub/OEBPS/document_1/document_1.html#_Toc172119266> ;
    dcat:landingPage "https://www.legislation.gov.au/C2020A00012/2024-07-10/2024-07-10/text/original/epub/OEBPS/document_1/document_1.html#_Toc172119266"^^xsd:anyURI ;
    dcat:theme legcons:Item .

C2020A00012:577 a legcons:Item,
        owl:Class,
        dcat:Resource ;
    rdfs:label "Item - I577 379 A  Simplified outline of this Part"@en-AU ;
    dct:isPartOf C2020A00012:576 ;
    dct:isReferencedBy C2020A00012: ;
    rdfs:comment "379 A  Simplified outline of this Part - Abrievated Graph Key: I577"@en-AU ;
    skos:definition "379 A  Simplified outline of this Part"@en-AU ;
    skos:narrower C2020A00012:576 ;
    skos:prefLabel "Item I577"@en-AU ;
    dcat:accessURL <https://www.legislation.gov.au/C2020A00012/2024-07-10/2024-07-10/text/original/epub/OEBPS/document_1/document_1.html#_Toc172119269> ;
    dcat:landingPage "https://www.legislation.gov.au/C2020A00012/2024-07-10/2024-07-10/text/original/epub/OEBPS/document_1/document_1.html#_Toc172119269"^^xsd:anyURI ;
    dcat:theme legcons:Item .

C2020A00012:579 a legcons:Item,
        owl:Class,
        dcat:Resource ;
    rdfs:label "Item - I579 379 B  Application to approve alternative regulatory arrangement"@en-AU ;
    dct:isPartOf C2020A00012:578 ;
    dct:isReferencedBy C2020A00012: ;
    rdfs:comment "379 B  Application to approve alternative regulatory arrangement - Abrievated Graph Key: I579"@en-AU ;
    skos:definition "379 B  Application to approve alternative regulatory arrangement"@en-AU ;
    skos:narrower C2020A00012:578 ;
    skos:prefLabel "Item I579"@en-AU ;
    dcat:accessURL <https://www.legislation.gov.au/C2020A00012/2024-07-10/2024-07-10/text/original/epub/OEBPS/document_1/document_1.html#_Toc172119271> ;
    dcat:landingPage "https://www.legislation.gov.au/C2020A00012/2024-07-10/2024-07-10/text/original/epub/OEBPS/document_1/document_1.html#_Toc172119271"^^xsd:anyURI ;
    dcat:theme legcons:Item .

C2020A00012:58 a legcons:Item,
        owl:Class,
        dcat:Resource ;
    rdfs:label "Item - I58 44  Exporting prescribed goods to a particular placenon compliance with prescribed export conditionseconomic consequences for Australia"@en-AU ;
    dct:isPartOf C2020A00012:28 ;
    dct:isReferencedBy C2020A00012: ;
    rdfs:comment "44  Exporting prescribed goods to a particular placenon compliance with prescribed export conditionseconomic consequences for Australia - Abrievated Graph Key: I58"@en-AU ;
    skos:definition "44  Exporting prescribed goods to a particular placenon compliance with prescribed export conditionseconomic consequences for Australia"@en-AU ;
    skos:narrower C2020A00012:28 ;
    skos:prefLabel "Item I58"@en-AU ;
    dcat:accessURL <https://www.legislation.gov.au/C2020A00012/2024-07-10/2024-07-10/text/original/epub/OEBPS/document_1/document_1.html#_Toc172118750> ;
    dcat:landingPage "https://www.legislation.gov.au/C2020A00012/2024-07-10/2024-07-10/text/original/epub/OEBPS/document_1/document_1.html#_Toc172118750"^^xsd:anyURI ;
    dcat:theme legcons:Item .

C2020A00012:580 a legcons:Item,
        owl:Class,
        dcat:Resource ;
    rdfs:label "Item - I580 379 C  Secretary must decide whether to approve alternative regulatory arrangement"@en-AU ;
    dct:isPartOf C2020A00012:578 ;
    dct:isReferencedBy C2020A00012: ;
    rdfs:comment "379 C  Secretary must decide whether to approve alternative regulatory arrangement - Abrievated Graph Key: I580"@en-AU ;
    skos:definition "379 C  Secretary must decide whether to approve alternative regulatory arrangement"@en-AU ;
    skos:narrower C2020A00012:578 ;
    skos:prefLabel "Item I580"@en-AU ;
    dcat:accessURL <https://www.legislation.gov.au/C2020A00012/2024-07-10/2024-07-10/text/original/epub/OEBPS/document_1/document_1.html#_Toc172119272> ;
    dcat:landingPage "https://www.legislation.gov.au/C2020A00012/2024-07-10/2024-07-10/text/original/epub/OEBPS/document_1/document_1.html#_Toc172119272"^^xsd:anyURI ;
    dcat:theme legcons:Item .

C2020A00012:583 a legcons:Item,
        owl:Class,
        dcat:Resource ;
    rdfs:label "Item - I583 380  Simplified outline of this Part"@en-AU ;
    dct:isPartOf C2020A00012:582 ;
    dct:isReferencedBy C2020A00012: ;
    rdfs:comment "380  Simplified outline of this Part - Abrievated Graph Key: I583"@en-AU ;
    skos:definition "380  Simplified outline of this Part"@en-AU ;
    skos:narrower C2020A00012:582 ;
    skos:prefLabel "Item I583"@en-AU ;
    dcat:accessURL <https://www.legislation.gov.au/C2020A00012/2024-07-10/2024-07-10/text/original/epub/OEBPS/document_1/document_1.html#_Toc172119275> ;
    dcat:landingPage "https://www.legislation.gov.au/C2020A00012/2024-07-10/2024-07-10/text/original/epub/OEBPS/document_1/document_1.html#_Toc172119275"^^xsd:anyURI ;
    dcat:theme legcons:Item .

C2020A00012:585 a legcons:Item,
        owl:Class,
        dcat:Resource ;
    rdfs:label "Item - I585 381  Reviewable decisions"@en-AU ;
    dct:isPartOf C2020A00012:584 ;
    dct:isReferencedBy C2020A00012: ;
    rdfs:comment "381  Reviewable decisions - Abrievated Graph Key: I585"@en-AU ;
    skos:definition "381  Reviewable decisions"@en-AU ;
    skos:narrower C2020A00012:584 ;
    skos:prefLabel "Item I585"@en-AU ;
    dcat:accessURL <https://www.legislation.gov.au/C2020A00012/2024-07-10/2024-07-10/text/original/epub/OEBPS/document_1/document_1.html#_Toc172119277> ;
    dcat:landingPage "https://www.legislation.gov.au/C2020A00012/2024-07-10/2024-07-10/text/original/epub/OEBPS/document_1/document_1.html#_Toc172119277"^^xsd:anyURI ;
    dcat:theme legcons:Item .

C2020A00012:586 a legcons:Item,
        owl:Class,
        dcat:Resource ;
    rdfs:label "Item - I586 382  Notice of decision"@en-AU ;
    dct:isPartOf C2020A00012:584 ;
    dct:isReferencedBy C2020A00012: ;
    rdfs:comment "382  Notice of decision - Abrievated Graph Key: I586"@en-AU ;
    skos:definition "382  Notice of decision"@en-AU ;
    skos:narrower C2020A00012:584 ;
    skos:prefLabel "Item I586"@en-AU ;
    dcat:accessURL <https://www.legislation.gov.au/C2020A00012/2024-07-10/2024-07-10/text/original/epub/OEBPS/document_1/document_1.html#_Toc172119278> ;
    dcat:landingPage "https://www.legislation.gov.au/C2020A00012/2024-07-10/2024-07-10/text/original/epub/OEBPS/document_1/document_1.html#_Toc172119278"^^xsd:anyURI ;
    dcat:theme legcons:Item .

C2020A00012:587 a legcons:Item,
        owl:Class,
        dcat:Resource ;
    rdfs:label "Item - I587 383  Internal review of reviewable decisions"@en-AU ;
    dct:isPartOf C2020A00012:584 ;
    dct:isReferencedBy C2020A00012: ;
    rdfs:comment "383  Internal review of reviewable decisions - Abrievated Graph Key: I587"@en-AU ;
    skos:definition "383  Internal review of reviewable decisions"@en-AU ;
    skos:narrower C2020A00012:584 ;
    skos:prefLabel "Item I587"@en-AU ;
    dcat:accessURL <https://www.legislation.gov.au/C2020A00012/2024-07-10/2024-07-10/text/original/epub/OEBPS/document_1/document_1.html#_Toc172119279> ;
    dcat:landingPage "https://www.legislation.gov.au/C2020A00012/2024-07-10/2024-07-10/text/original/epub/OEBPS/document_1/document_1.html#_Toc172119279"^^xsd:anyURI ;
    dcat:theme legcons:Item .

C2020A00012:588 a legcons:Item,
        owl:Class,
        dcat:Resource ;
    rdfs:label "Item - I588 384  Secretary may require further information from applicants"@en-AU ;
    dct:isPartOf C2020A00012:584 ;
    dct:isReferencedBy C2020A00012: ;
    rdfs:comment "384  Secretary may require further information from applicants - Abrievated Graph Key: I588"@en-AU ;
    skos:definition "384  Secretary may require further information from applicants"@en-AU ;
    skos:narrower C2020A00012:584 ;
    skos:prefLabel "Item I588"@en-AU ;
    dcat:accessURL <https://www.legislation.gov.au/C2020A00012/2024-07-10/2024-07-10/text/original/epub/OEBPS/document_1/document_1.html#_Toc172119280> ;
    dcat:landingPage "https://www.legislation.gov.au/C2020A00012/2024-07-10/2024-07-10/text/original/epub/OEBPS/document_1/document_1.html#_Toc172119280"^^xsd:anyURI ;
    dcat:theme legcons:Item .

C2020A00012:589 a legcons:Item,
        owl:Class,
        dcat:Resource ;
    rdfs:label "Item - I589 385  Review by the Administrative Appeals Tribunal"@en-AU ;
    dct:isPartOf C2020A00012:584 ;
    dct:isReferencedBy C2020A00012: ;
    rdfs:comment "385  Review by the Administrative Appeals Tribunal - Abrievated Graph Key: I589"@en-AU ;
    skos:definition "385  Review by the Administrative Appeals Tribunal"@en-AU ;
    skos:narrower C2020A00012:584 ;
    skos:prefLabel "Item I589"@en-AU ;
    dcat:accessURL <https://www.legislation.gov.au/C2020A00012/2024-07-10/2024-07-10/text/original/epub/OEBPS/document_1/document_1.html#_Toc172119281> ;
    dcat:landingPage "https://www.legislation.gov.au/C2020A00012/2024-07-10/2024-07-10/text/original/epub/OEBPS/document_1/document_1.html#_Toc172119281"^^xsd:anyURI ;
    dcat:theme legcons:Item .

C2020A00012:59 a legcons:Item,
        owl:Class,
        dcat:Resource ;
    rdfs:label "Item - I59 45  Conveying or possessing prescribed goods that are intended to be exported to a particular place in contravention of conditions etc"@en-AU ;
    dct:isPartOf C2020A00012:28 ;
    dct:isReferencedBy C2020A00012: ;
    rdfs:comment "45  Conveying or possessing prescribed goods that are intended to be exported to a particular place in contravention of conditions etc - Abrievated Graph Key: I59"@en-AU ;
    skos:definition "45  Conveying or possessing prescribed goods that are intended to be exported to a particular place in contravention of conditions etc"@en-AU ;
    skos:narrower C2020A00012:28 ;
    skos:prefLabel "Item I59"@en-AU ;
    dcat:accessURL <https://www.legislation.gov.au/C2020A00012/2024-07-10/2024-07-10/text/original/epub/OEBPS/document_1/document_1.html#_Toc172118751> ;
    dcat:landingPage "https://www.legislation.gov.au/C2020A00012/2024-07-10/2024-07-10/text/original/epub/OEBPS/document_1/document_1.html#_Toc172118751"^^xsd:anyURI ;
    dcat:theme legcons:Item .

C2020A00012:590 a legcons:Item,
        owl:Class,
        dcat:Resource ;
    rdfs:label "Item - I590 386  Review of decisions relating to tariff rate quota entitlements or tariff rate quota certificates"@en-AU ;
    dct:isPartOf C2020A00012:584 ;
    dct:isReferencedBy C2020A00012: ;
    rdfs:comment "386  Review of decisions relating to tariff rate quota entitlements or tariff rate quota certificates - Abrievated Graph Key: I590"@en-AU ;
    skos:definition "386  Review of decisions relating to tariff rate quota entitlements or tariff rate quota certificates"@en-AU ;
    skos:narrower C2020A00012:584 ;
    skos:prefLabel "Item I590"@en-AU ;
    dcat:accessURL <https://www.legislation.gov.au/C2020A00012/2024-07-10/2024-07-10/text/original/epub/OEBPS/document_1/document_1.html#_Toc172119282> ;
    dcat:landingPage "https://www.legislation.gov.au/C2020A00012/2024-07-10/2024-07-10/text/original/epub/OEBPS/document_1/document_1.html#_Toc172119282"^^xsd:anyURI ;
    dcat:theme legcons:Item .

C2020A00012:593 a legcons:Item,
        owl:Class,
        dcat:Resource ;
    rdfs:label "Item - I593 387  Simplified outline of this Part"@en-AU ;
    dct:isPartOf C2020A00012:592 ;
    dct:isReferencedBy C2020A00012: ;
    rdfs:comment "387  Simplified outline of this Part - Abrievated Graph Key: I593"@en-AU ;
    skos:definition "387  Simplified outline of this Part"@en-AU ;
    skos:narrower C2020A00012:592 ;
    skos:prefLabel "Item I593"@en-AU ;
    dcat:accessURL <https://www.legislation.gov.au/C2020A00012/2024-07-10/2024-07-10/text/original/epub/OEBPS/document_1/document_1.html#_Toc172119285> ;
    dcat:landingPage "https://www.legislation.gov.au/C2020A00012/2024-07-10/2024-07-10/text/original/epub/OEBPS/document_1/document_1.html#_Toc172119285"^^xsd:anyURI ;
    dcat:theme legcons:Item .

C2020A00012:595 a legcons:Item,
        owl:Class,
        dcat:Resource ;
    rdfs:label "Item - I595 388  Use or disclosure for the purposes of this Act"@en-AU ;
    dct:isPartOf C2020A00012:594 ;
    dct:isReferencedBy C2020A00012: ;
    rdfs:comment "388  Use or disclosure for the purposes of this Act - Abrievated Graph Key: I595"@en-AU ;
    skos:definition "388  Use or disclosure for the purposes of this Act"@en-AU ;
    skos:narrower C2020A00012:594 ;
    skos:prefLabel "Item I595"@en-AU ;
    dcat:accessURL <https://www.legislation.gov.au/C2020A00012/2024-07-10/2024-07-10/text/original/epub/OEBPS/document_1/document_1.html#_Toc172119287> ;
    dcat:landingPage "https://www.legislation.gov.au/C2020A00012/2024-07-10/2024-07-10/text/original/epub/OEBPS/document_1/document_1.html#_Toc172119287"^^xsd:anyURI ;
    dcat:theme legcons:Item .

C2020A00012:596 a legcons:Item,
        owl:Class,
        dcat:Resource ;
    rdfs:label "Item - I596 389  Disclosure to foreign governments etc for export trade and other purposes"@en-AU ;
    dct:isPartOf C2020A00012:594 ;
    dct:isReferencedBy C2020A00012: ;
    rdfs:comment "389  Disclosure to foreign governments etc for export trade and other purposes - Abrievated Graph Key: I596"@en-AU ;
    skos:definition "389  Disclosure to foreign governments etc for export trade and other purposes"@en-AU ;
    skos:narrower C2020A00012:594 ;
    skos:prefLabel "Item I596"@en-AU ;
    dcat:accessURL <https://www.legislation.gov.au/C2020A00012/2024-07-10/2024-07-10/text/original/epub/OEBPS/document_1/document_1.html#_Toc172119288> ;
    dcat:landingPage "https://www.legislation.gov.au/C2020A00012/2024-07-10/2024-07-10/text/original/epub/OEBPS/document_1/document_1.html#_Toc172119288"^^xsd:anyURI ;
    dcat:theme legcons:Item .

C2020A00012:597 a legcons:Item,
        owl:Class,
        dcat:Resource ;
    rdfs:label "Item - I597 390  Use or disclosure for the purposes of certain Acts"@en-AU ;
    dct:isPartOf C2020A00012:594 ;
    dct:isReferencedBy C2020A00012: ;
    rdfs:comment "390  Use or disclosure for the purposes of certain Acts - Abrievated Graph Key: I597"@en-AU ;
    skos:definition "390  Use or disclosure for the purposes of certain Acts"@en-AU ;
    skos:narrower C2020A00012:594 ;
    skos:prefLabel "Item I597"@en-AU ;
    dcat:accessURL <https://www.legislation.gov.au/C2020A00012/2024-07-10/2024-07-10/text/original/epub/OEBPS/document_1/document_1.html#_Toc172119289> ;
    dcat:landingPage "https://www.legislation.gov.au/C2020A00012/2024-07-10/2024-07-10/text/original/epub/OEBPS/document_1/document_1.html#_Toc172119289"^^xsd:anyURI ;
    dcat:theme legcons:Item .

C2020A00012:598 a legcons:Item,
        owl:Class,
        dcat:Resource ;
    rdfs:label "Item - I598 391  Disclosure to a Commonwealth entity"@en-AU ;
    dct:isPartOf C2020A00012:594 ;
    dct:isReferencedBy C2020A00012: ;
    rdfs:comment "391  Disclosure to a Commonwealth entity - Abrievated Graph Key: I598"@en-AU ;
    skos:definition "391  Disclosure to a Commonwealth entity"@en-AU ;
    skos:narrower C2020A00012:594 ;
    skos:prefLabel "Item I598"@en-AU ;
    dcat:accessURL <https://www.legislation.gov.au/C2020A00012/2024-07-10/2024-07-10/text/original/epub/OEBPS/document_1/document_1.html#_Toc172119290> ;
    dcat:landingPage "https://www.legislation.gov.au/C2020A00012/2024-07-10/2024-07-10/text/original/epub/OEBPS/document_1/document_1.html#_Toc172119290"^^xsd:anyURI ;
    dcat:theme legcons:Item .

C2020A00012:599 a legcons:Item,
        owl:Class,
        dcat:Resource ;
    rdfs:label "Item - I599 392  Disclosure to a court tribunal etc"@en-AU ;
    dct:isPartOf C2020A00012:594 ;
    dct:isReferencedBy C2020A00012: ;
    rdfs:comment "392  Disclosure to a court tribunal etc - Abrievated Graph Key: I599"@en-AU ;
    skos:definition "392  Disclosure to a court tribunal etc"@en-AU ;
    skos:narrower C2020A00012:594 ;
    skos:prefLabel "Item I599"@en-AU ;
    dcat:accessURL <https://www.legislation.gov.au/C2020A00012/2024-07-10/2024-07-10/text/original/epub/OEBPS/document_1/document_1.html#_Toc172119291> ;
    dcat:landingPage "https://www.legislation.gov.au/C2020A00012/2024-07-10/2024-07-10/text/original/epub/OEBPS/document_1/document_1.html#_Toc172119291"^^xsd:anyURI ;
    dcat:theme legcons:Item .

C2020A00012:6 a legcons:Item,
        owl:Class,
        dcat:Resource ;
    rdfs:label "Item - I6 4  Simplified outline of this Act"@en-AU ;
    dct:isPartOf C2020A00012:1 ;
    dct:isReferencedBy C2020A00012: ;
    rdfs:comment "4  Simplified outline of this Act - Abrievated Graph Key: I6"@en-AU ;
    skos:definition "4  Simplified outline of this Act"@en-AU ;
    skos:narrower C2020A00012:1 ;
    skos:prefLabel "Item I6"@en-AU ;
    dcat:accessURL <https://www.legislation.gov.au/C2020A00012/2024-07-10/2024-07-10/text/original/epub/OEBPS/document_1/document_1.html#_Toc172118698> ;
    dcat:landingPage "https://www.legislation.gov.au/C2020A00012/2024-07-10/2024-07-10/text/original/epub/OEBPS/document_1/document_1.html#_Toc172118698"^^xsd:anyURI ;
    dcat:theme legcons:Item .

C2020A00012:60 a legcons:Item,
        owl:Class,
        dcat:Resource ;
    rdfs:label "Item - I60 46  Producing or preparing prescribed goods or other goods at certain premises in contravention of conditionsgeneral"@en-AU ;
    dct:isPartOf C2020A00012:28 ;
    dct:isReferencedBy C2020A00012: ;
    rdfs:comment "46  Producing or preparing prescribed goods or other goods at certain premises in contravention of conditionsgeneral - Abrievated Graph Key: I60"@en-AU ;
    skos:definition "46  Producing or preparing prescribed goods or other goods at certain premises in contravention of conditionsgeneral"@en-AU ;
    skos:narrower C2020A00012:28 ;
    skos:prefLabel "Item I60"@en-AU ;
    dcat:accessURL <https://www.legislation.gov.au/C2020A00012/2024-07-10/2024-07-10/text/original/epub/OEBPS/document_1/document_1.html#_Toc172118752> ;
    dcat:landingPage "https://www.legislation.gov.au/C2020A00012/2024-07-10/2024-07-10/text/original/epub/OEBPS/document_1/document_1.html#_Toc172118752"^^xsd:anyURI ;
    dcat:theme legcons:Item .

C2020A00012:600 a legcons:Item,
        owl:Class,
        dcat:Resource ;
    rdfs:label "Item - I600 393  Disclosure for the purposes of law enforcement"@en-AU ;
    dct:isPartOf C2020A00012:594 ;
    dct:isReferencedBy C2020A00012: ;
    rdfs:comment "393  Disclosure for the purposes of law enforcement - Abrievated Graph Key: I600"@en-AU ;
    skos:definition "393  Disclosure for the purposes of law enforcement"@en-AU ;
    skos:narrower C2020A00012:594 ;
    skos:prefLabel "Item I600"@en-AU ;
    dcat:accessURL <https://www.legislation.gov.au/C2020A00012/2024-07-10/2024-07-10/text/original/epub/OEBPS/document_1/document_1.html#_Toc172119292> ;
    dcat:landingPage "https://www.legislation.gov.au/C2020A00012/2024-07-10/2024-07-10/text/original/epub/OEBPS/document_1/document_1.html#_Toc172119292"^^xsd:anyURI ;
    dcat:theme legcons:Item .

C2020A00012:601 a legcons:Item,
        owl:Class,
        dcat:Resource ;
    rdfs:label "Item - I601 394  Use or disclosure for research policy development or data analysis"@en-AU ;
    dct:isPartOf C2020A00012:594 ;
    dct:isReferencedBy C2020A00012: ;
    rdfs:comment "394  Use or disclosure for research policy development or data analysis - Abrievated Graph Key: I601"@en-AU ;
    skos:definition "394  Use or disclosure for research policy development or data analysis"@en-AU ;
    skos:narrower C2020A00012:594 ;
    skos:prefLabel "Item I601"@en-AU ;
    dcat:accessURL <https://www.legislation.gov.au/C2020A00012/2024-07-10/2024-07-10/text/original/epub/OEBPS/document_1/document_1.html#_Toc172119293> ;
    dcat:landingPage "https://www.legislation.gov.au/C2020A00012/2024-07-10/2024-07-10/text/original/epub/OEBPS/document_1/document_1.html#_Toc172119293"^^xsd:anyURI ;
    dcat:theme legcons:Item .

C2020A00012:602 a legcons:Item,
        owl:Class,
        dcat:Resource ;
    rdfs:label "Item - I602 395  Use or disclosure of statistics"@en-AU ;
    dct:isPartOf C2020A00012:594 ;
    dct:isReferencedBy C2020A00012: ;
    rdfs:comment "395  Use or disclosure of statistics - Abrievated Graph Key: I602"@en-AU ;
    skos:definition "395  Use or disclosure of statistics"@en-AU ;
    skos:narrower C2020A00012:594 ;
    skos:prefLabel "Item I602"@en-AU ;
    dcat:accessURL <https://www.legislation.gov.au/C2020A00012/2024-07-10/2024-07-10/text/original/epub/OEBPS/document_1/document_1.html#_Toc172119294> ;
    dcat:landingPage "https://www.legislation.gov.au/C2020A00012/2024-07-10/2024-07-10/text/original/epub/OEBPS/document_1/document_1.html#_Toc172119294"^^xsd:anyURI ;
    dcat:theme legcons:Item .

C2020A00012:603 a legcons:Item,
        owl:Class,
        dcat:Resource ;
    rdfs:label "Item - I603 396  Use or disclosure of publicly available information"@en-AU ;
    dct:isPartOf C2020A00012:594 ;
    dct:isReferencedBy C2020A00012: ;
    rdfs:comment "396  Use or disclosure of publicly available information - Abrievated Graph Key: I603"@en-AU ;
    skos:definition "396  Use or disclosure of publicly available information"@en-AU ;
    skos:narrower C2020A00012:594 ;
    skos:prefLabel "Item I603"@en-AU ;
    dcat:accessURL <https://www.legislation.gov.au/C2020A00012/2024-07-10/2024-07-10/text/original/epub/OEBPS/document_1/document_1.html#_Toc172119295> ;
    dcat:landingPage "https://www.legislation.gov.au/C2020A00012/2024-07-10/2024-07-10/text/original/epub/OEBPS/document_1/document_1.html#_Toc172119295"^^xsd:anyURI ;
    dcat:theme legcons:Item .

C2020A00012:604 a legcons:Item,
        owl:Class,
        dcat:Resource ;
    rdfs:label "Item - I604 397  Disclosure to person to whom information relates"@en-AU ;
    dct:isPartOf C2020A00012:594 ;
    dct:isReferencedBy C2020A00012: ;
    rdfs:comment "397  Disclosure to person to whom information relates - Abrievated Graph Key: I604"@en-AU ;
    skos:definition "397  Disclosure to person to whom information relates"@en-AU ;
    skos:narrower C2020A00012:594 ;
    skos:prefLabel "Item I604"@en-AU ;
    dcat:accessURL <https://www.legislation.gov.au/C2020A00012/2024-07-10/2024-07-10/text/original/epub/OEBPS/document_1/document_1.html#_Toc172119296> ;
    dcat:landingPage "https://www.legislation.gov.au/C2020A00012/2024-07-10/2024-07-10/text/original/epub/OEBPS/document_1/document_1.html#_Toc172119296"^^xsd:anyURI ;
    dcat:theme legcons:Item .

C2020A00012:605 a legcons:Item,
        owl:Class,
        dcat:Resource ;
    rdfs:label "Item - I605 397 A  Use or disclosure with consent"@en-AU ;
    dct:isPartOf C2020A00012:594 ;
    dct:isReferencedBy C2020A00012: ;
    rdfs:comment "397 A  Use or disclosure with consent - Abrievated Graph Key: I605"@en-AU ;
    skos:definition "397 A  Use or disclosure with consent"@en-AU ;
    skos:narrower C2020A00012:594 ;
    skos:prefLabel "Item I605"@en-AU ;
    dcat:accessURL <https://www.legislation.gov.au/C2020A00012/2024-07-10/2024-07-10/text/original/epub/OEBPS/document_1/document_1.html#_Toc172119297> ;
    dcat:landingPage "https://www.legislation.gov.au/C2020A00012/2024-07-10/2024-07-10/text/original/epub/OEBPS/document_1/document_1.html#_Toc172119297"^^xsd:anyURI ;
    dcat:theme legcons:Item .

C2020A00012:606 a legcons:Item,
        owl:Class,
        dcat:Resource ;
    rdfs:label "Item - I606 397 B  Disclosure to person who provided information"@en-AU ;
    dct:isPartOf C2020A00012:594 ;
    dct:isReferencedBy C2020A00012: ;
    rdfs:comment "397 B  Disclosure to person who provided information - Abrievated Graph Key: I606"@en-AU ;
    skos:definition "397 B  Disclosure to person who provided information"@en-AU ;
    skos:narrower C2020A00012:594 ;
    skos:prefLabel "Item I606"@en-AU ;
    dcat:accessURL <https://www.legislation.gov.au/C2020A00012/2024-07-10/2024-07-10/text/original/epub/OEBPS/document_1/document_1.html#_Toc172119298> ;
    dcat:landingPage "https://www.legislation.gov.au/C2020A00012/2024-07-10/2024-07-10/text/original/epub/OEBPS/document_1/document_1.html#_Toc172119298"^^xsd:anyURI ;
    dcat:theme legcons:Item .

C2020A00012:607 a legcons:Item,
        owl:Class,
        dcat:Resource ;
    rdfs:label "Item - I607 397 C  Disclosure to State or Territory body"@en-AU ;
    dct:isPartOf C2020A00012:594 ;
    dct:isReferencedBy C2020A00012: ;
    rdfs:comment "397 C  Disclosure to State or Territory body - Abrievated Graph Key: I607"@en-AU ;
    skos:definition "397 C  Disclosure to State or Territory body"@en-AU ;
    skos:narrower C2020A00012:594 ;
    skos:prefLabel "Item I607"@en-AU ;
    dcat:accessURL <https://www.legislation.gov.au/C2020A00012/2024-07-10/2024-07-10/text/original/epub/OEBPS/document_1/document_1.html#_Toc172119299> ;
    dcat:landingPage "https://www.legislation.gov.au/C2020A00012/2024-07-10/2024-07-10/text/original/epub/OEBPS/document_1/document_1.html#_Toc172119299"^^xsd:anyURI ;
    dcat:theme legcons:Item .

C2020A00012:608 a legcons:Item,
        owl:Class,
        dcat:Resource ;
    rdfs:label "Item - I608 397 D  Use or disclosure to manage severe and immediate threats"@en-AU ;
    dct:isPartOf C2020A00012:594 ;
    dct:isReferencedBy C2020A00012: ;
    rdfs:comment "397 D  Use or disclosure to manage severe and immediate threats - Abrievated Graph Key: I608"@en-AU ;
    skos:definition "397 D  Use or disclosure to manage severe and immediate threats"@en-AU ;
    skos:narrower C2020A00012:594 ;
    skos:prefLabel "Item I608"@en-AU ;
    dcat:accessURL <https://www.legislation.gov.au/C2020A00012/2024-07-10/2024-07-10/text/original/epub/OEBPS/document_1/document_1.html#_Toc172119300> ;
    dcat:landingPage "https://www.legislation.gov.au/C2020A00012/2024-07-10/2024-07-10/text/original/epub/OEBPS/document_1/document_1.html#_Toc172119300"^^xsd:anyURI ;
    dcat:theme legcons:Item .

C2020A00012:609 a legcons:Item,
        owl:Class,
        dcat:Resource ;
    rdfs:label "Item - I609 397 E  Use or disclosure authorised by rules"@en-AU ;
    dct:isPartOf C2020A00012:594 ;
    dct:isReferencedBy C2020A00012: ;
    rdfs:comment "397 E  Use or disclosure authorised by rules - Abrievated Graph Key: I609"@en-AU ;
    skos:definition "397 E  Use or disclosure authorised by rules"@en-AU ;
    skos:narrower C2020A00012:594 ;
    skos:prefLabel "Item I609"@en-AU ;
    dcat:accessURL <https://www.legislation.gov.au/C2020A00012/2024-07-10/2024-07-10/text/original/epub/OEBPS/document_1/document_1.html#_Toc172119301> ;
    dcat:landingPage "https://www.legislation.gov.au/C2020A00012/2024-07-10/2024-07-10/text/original/epub/OEBPS/document_1/document_1.html#_Toc172119301"^^xsd:anyURI ;
    dcat:theme legcons:Item .

C2020A00012:61 a legcons:Item,
        owl:Class,
        dcat:Resource ;
    rdfs:label "Item - I61 47  Producing or preparing prescribed goods or other goods at certain premises in contravention of conditionsgoods to be exported to a particular place"@en-AU ;
    dct:isPartOf C2020A00012:28 ;
    dct:isReferencedBy C2020A00012: ;
    rdfs:comment "47  Producing or preparing prescribed goods or other goods at certain premises in contravention of conditionsgoods to be exported to a particular place - Abrievated Graph Key: I61"@en-AU ;
    skos:definition "47  Producing or preparing prescribed goods or other goods at certain premises in contravention of conditionsgoods to be exported to a particular place"@en-AU ;
    skos:narrower C2020A00012:28 ;
    skos:prefLabel "Item I61"@en-AU ;
    dcat:accessURL <https://www.legislation.gov.au/C2020A00012/2024-07-10/2024-07-10/text/original/epub/OEBPS/document_1/document_1.html#_Toc172118753> ;
    dcat:landingPage "https://www.legislation.gov.au/C2020A00012/2024-07-10/2024-07-10/text/original/epub/OEBPS/document_1/document_1.html#_Toc172118753"^^xsd:anyURI ;
    dcat:theme legcons:Item .

C2020A00012:611 a legcons:Item,
        owl:Class,
        dcat:Resource ;
    rdfs:label "Item - I611 397 F  Meaning of protected information"@en-AU ;
    dct:isPartOf C2020A00012:610 ;
    dct:isReferencedBy C2020A00012: ;
    rdfs:comment "397 F  Meaning of protected information - Abrievated Graph Key: I611"@en-AU ;
    skos:definition "397 F  Meaning of protected information"@en-AU ;
    skos:narrower C2020A00012:610 ;
    skos:prefLabel "Item I611"@en-AU ;
    dcat:accessURL <https://www.legislation.gov.au/C2020A00012/2024-07-10/2024-07-10/text/original/epub/OEBPS/document_1/document_1.html#_Toc172119303> ;
    dcat:landingPage "https://www.legislation.gov.au/C2020A00012/2024-07-10/2024-07-10/text/original/epub/OEBPS/document_1/document_1.html#_Toc172119303"^^xsd:anyURI ;
    dcat:theme legcons:Item .

C2020A00012:612 a legcons:Item,
        owl:Class,
        dcat:Resource ;
    rdfs:label "Item - I612 397 G  Offence and civil penaltyuse or disclosure of protected information"@en-AU ;
    dct:isPartOf C2020A00012:610 ;
    dct:isReferencedBy C2020A00012: ;
    rdfs:comment "397 G  Offence and civil penaltyuse or disclosure of protected information - Abrievated Graph Key: I612"@en-AU ;
    skos:definition "397 G  Offence and civil penaltyuse or disclosure of protected information"@en-AU ;
    skos:narrower C2020A00012:610 ;
    skos:prefLabel "Item I612"@en-AU ;
    dcat:accessURL <https://www.legislation.gov.au/C2020A00012/2024-07-10/2024-07-10/text/original/epub/OEBPS/document_1/document_1.html#_Toc172119304> ;
    dcat:landingPage "https://www.legislation.gov.au/C2020A00012/2024-07-10/2024-07-10/text/original/epub/OEBPS/document_1/document_1.html#_Toc172119304"^^xsd:anyURI ;
    dcat:theme legcons:Item .

C2020A00012:615 a legcons:Item,
        owl:Class,
        dcat:Resource ;
    rdfs:label "Item - I615 398  Simplified outline of this Part"@en-AU ;
    dct:isPartOf C2020A00012:614 ;
    dct:isReferencedBy C2020A00012: ;
    rdfs:comment "398  Simplified outline of this Part - Abrievated Graph Key: I615"@en-AU ;
    skos:definition "398  Simplified outline of this Part"@en-AU ;
    skos:narrower C2020A00012:614 ;
    skos:prefLabel "Item I615"@en-AU ;
    dcat:accessURL <https://www.legislation.gov.au/C2020A00012/2024-07-10/2024-07-10/text/original/epub/OEBPS/document_1/document_1.html#_Toc172119307> ;
    dcat:landingPage "https://www.legislation.gov.au/C2020A00012/2024-07-10/2024-07-10/text/original/epub/OEBPS/document_1/document_1.html#_Toc172119307"^^xsd:anyURI ;
    dcat:theme legcons:Item .

C2020A00012:617 a legcons:Item,
        owl:Class,
        dcat:Resource ;
    rdfs:label "Item - I617 399  Fees and other rules for fee bearing activities"@en-AU ;
    dct:isPartOf C2020A00012:616 ;
    dct:isReferencedBy C2020A00012: ;
    rdfs:comment "399  Fees and other rules for fee bearing activities - Abrievated Graph Key: I617"@en-AU ;
    skos:definition "399  Fees and other rules for fee bearing activities"@en-AU ;
    skos:narrower C2020A00012:616 ;
    skos:prefLabel "Item I617"@en-AU ;
    dcat:accessURL <https://www.legislation.gov.au/C2020A00012/2024-07-10/2024-07-10/text/original/epub/OEBPS/document_1/document_1.html#_Toc172119309> ;
    dcat:landingPage "https://www.legislation.gov.au/C2020A00012/2024-07-10/2024-07-10/text/original/epub/OEBPS/document_1/document_1.html#_Toc172119309"^^xsd:anyURI ;
    dcat:theme legcons:Item .

C2020A00012:619 a legcons:Item,
        owl:Class,
        dcat:Resource ;
    rdfs:label "Item - I619 400  Paying cost recovery charges"@en-AU ;
    dct:isPartOf C2020A00012:618 ;
    dct:isReferencedBy C2020A00012: ;
    rdfs:comment "400  Paying cost recovery charges - Abrievated Graph Key: I619"@en-AU ;
    skos:definition "400  Paying cost recovery charges"@en-AU ;
    skos:narrower C2020A00012:618 ;
    skos:prefLabel "Item I619"@en-AU ;
    dcat:accessURL <https://www.legislation.gov.au/C2020A00012/2024-07-10/2024-07-10/text/original/epub/OEBPS/document_1/document_1.html#_Toc172119311> ;
    dcat:landingPage "https://www.legislation.gov.au/C2020A00012/2024-07-10/2024-07-10/text/original/epub/OEBPS/document_1/document_1.html#_Toc172119311"^^xsd:anyURI ;
    dcat:theme legcons:Item .

C2020A00012:62 a legcons:Item,
        owl:Class,
        dcat:Resource ;
    rdfs:label "Item - I62 48  Making false or misleading representation about prescribed goods that are entered for exportgeneral"@en-AU ;
    dct:isPartOf C2020A00012:28 ;
    dct:isReferencedBy C2020A00012: ;
    rdfs:comment "48  Making false or misleading representation about prescribed goods that are entered for exportgeneral - Abrievated Graph Key: I62"@en-AU ;
    skos:definition "48  Making false or misleading representation about prescribed goods that are entered for exportgeneral"@en-AU ;
    skos:narrower C2020A00012:28 ;
    skos:prefLabel "Item I62"@en-AU ;
    dcat:accessURL <https://www.legislation.gov.au/C2020A00012/2024-07-10/2024-07-10/text/original/epub/OEBPS/document_1/document_1.html#_Toc172118754> ;
    dcat:landingPage "https://www.legislation.gov.au/C2020A00012/2024-07-10/2024-07-10/text/original/epub/OEBPS/document_1/document_1.html#_Toc172118754"^^xsd:anyURI ;
    dcat:theme legcons:Item .

C2020A00012:620 a legcons:Item,
        owl:Class,
        dcat:Resource ;
    rdfs:label "Item - I620 401  Person liable to pay cost recovery charges"@en-AU ;
    dct:isPartOf C2020A00012:618 ;
    dct:isReferencedBy C2020A00012: ;
    rdfs:comment "401  Person liable to pay cost recovery charges - Abrievated Graph Key: I620"@en-AU ;
    skos:definition "401  Person liable to pay cost recovery charges"@en-AU ;
    skos:narrower C2020A00012:618 ;
    skos:prefLabel "Item I620"@en-AU ;
    dcat:accessURL <https://www.legislation.gov.au/C2020A00012/2024-07-10/2024-07-10/text/original/epub/OEBPS/document_1/document_1.html#_Toc172119312> ;
    dcat:landingPage "https://www.legislation.gov.au/C2020A00012/2024-07-10/2024-07-10/text/original/epub/OEBPS/document_1/document_1.html#_Toc172119312"^^xsd:anyURI ;
    dcat:theme legcons:Item .

C2020A00012:621 a legcons:Item,
        owl:Class,
        dcat:Resource ;
    rdfs:label "Item - I621 402  Notional payments by the Commonwealth"@en-AU ;
    dct:isPartOf C2020A00012:618 ;
    dct:isReferencedBy C2020A00012: ;
    rdfs:comment "402  Notional payments by the Commonwealth - Abrievated Graph Key: I621"@en-AU ;
    skos:definition "402  Notional payments by the Commonwealth"@en-AU ;
    skos:narrower C2020A00012:618 ;
    skos:prefLabel "Item I621"@en-AU ;
    dcat:accessURL <https://www.legislation.gov.au/C2020A00012/2024-07-10/2024-07-10/text/original/epub/OEBPS/document_1/document_1.html#_Toc172119313> ;
    dcat:landingPage "https://www.legislation.gov.au/C2020A00012/2024-07-10/2024-07-10/text/original/epub/OEBPS/document_1/document_1.html#_Toc172119313"^^xsd:anyURI ;
    dcat:theme legcons:Item .

C2020A00012:623 a legcons:Item,
        owl:Class,
        dcat:Resource ;
    rdfs:label "Item - I623 403  Late payment fee"@en-AU ;
    dct:isPartOf C2020A00012:622 ;
    dct:isReferencedBy C2020A00012: ;
    rdfs:comment "403  Late payment fee - Abrievated Graph Key: I623"@en-AU ;
    skos:definition "403  Late payment fee"@en-AU ;
    skos:narrower C2020A00012:622 ;
    skos:prefLabel "Item I623"@en-AU ;
    dcat:accessURL <https://www.legislation.gov.au/C2020A00012/2024-07-10/2024-07-10/text/original/epub/OEBPS/document_1/document_1.html#_Toc172119315> ;
    dcat:landingPage "https://www.legislation.gov.au/C2020A00012/2024-07-10/2024-07-10/text/original/epub/OEBPS/document_1/document_1.html#_Toc172119315"^^xsd:anyURI ;
    dcat:theme legcons:Item .

C2020A00012:624 a legcons:Item,
        owl:Class,
        dcat:Resource ;
    rdfs:label "Item - I624 404  Recovery of cost recovery charges"@en-AU ;
    dct:isPartOf C2020A00012:622 ;
    dct:isReferencedBy C2020A00012: ;
    rdfs:comment "404  Recovery of cost recovery charges - Abrievated Graph Key: I624"@en-AU ;
    skos:definition "404  Recovery of cost recovery charges"@en-AU ;
    skos:narrower C2020A00012:622 ;
    skos:prefLabel "Item I624"@en-AU ;
    dcat:accessURL <https://www.legislation.gov.au/C2020A00012/2024-07-10/2024-07-10/text/original/epub/OEBPS/document_1/document_1.html#_Toc172119316> ;
    dcat:landingPage "https://www.legislation.gov.au/C2020A00012/2024-07-10/2024-07-10/text/original/epub/OEBPS/document_1/document_1.html#_Toc172119316"^^xsd:anyURI ;
    dcat:theme legcons:Item .

C2020A00012:626 a legcons:Item,
        owl:Class,
        dcat:Resource ;
    rdfs:label "Item - I626 405  Secretary may remit or refund cost recovery charges"@en-AU ;
    dct:isPartOf C2020A00012:625 ;
    dct:isReferencedBy C2020A00012: ;
    rdfs:comment "405  Secretary may remit or refund cost recovery charges - Abrievated Graph Key: I626"@en-AU ;
    skos:definition "405  Secretary may remit or refund cost recovery charges"@en-AU ;
    skos:narrower C2020A00012:625 ;
    skos:prefLabel "Item I626"@en-AU ;
    dcat:accessURL <https://www.legislation.gov.au/C2020A00012/2024-07-10/2024-07-10/text/original/epub/OEBPS/document_1/document_1.html#_Toc172119318> ;
    dcat:landingPage "https://www.legislation.gov.au/C2020A00012/2024-07-10/2024-07-10/text/original/epub/OEBPS/document_1/document_1.html#_Toc172119318"^^xsd:anyURI ;
    dcat:theme legcons:Item .

C2020A00012:627 a legcons:Item,
        owl:Class,
        dcat:Resource ;
    rdfs:label "Item - I627 406  Secretary may direct that activities not be carried out"@en-AU ;
    dct:isPartOf C2020A00012:625 ;
    dct:isReferencedBy C2020A00012: ;
    rdfs:comment "406  Secretary may direct that activities not be carried out - Abrievated Graph Key: I627"@en-AU ;
    skos:definition "406  Secretary may direct that activities not be carried out"@en-AU ;
    skos:narrower C2020A00012:625 ;
    skos:prefLabel "Item I627"@en-AU ;
    dcat:accessURL <https://www.legislation.gov.au/C2020A00012/2024-07-10/2024-07-10/text/original/epub/OEBPS/document_1/document_1.html#_Toc172119319> ;
    dcat:landingPage "https://www.legislation.gov.au/C2020A00012/2024-07-10/2024-07-10/text/original/epub/OEBPS/document_1/document_1.html#_Toc172119319"^^xsd:anyURI ;
    dcat:theme legcons:Item .

C2020A00012:63 a legcons:Item,
        owl:Class,
        dcat:Resource ;
    rdfs:label "Item - I63 49  Making false or misleading representation about prescribed goods that are entered for export to a particular place"@en-AU ;
    dct:isPartOf C2020A00012:28 ;
    dct:isReferencedBy C2020A00012: ;
    rdfs:comment "49  Making false or misleading representation about prescribed goods that are entered for export to a particular place - Abrievated Graph Key: I63"@en-AU ;
    skos:definition "49  Making false or misleading representation about prescribed goods that are entered for export to a particular place"@en-AU ;
    skos:narrower C2020A00012:28 ;
    skos:prefLabel "Item I63"@en-AU ;
    dcat:accessURL <https://www.legislation.gov.au/C2020A00012/2024-07-10/2024-07-10/text/original/epub/OEBPS/document_1/document_1.html#_Toc172118755> ;
    dcat:landingPage "https://www.legislation.gov.au/C2020A00012/2024-07-10/2024-07-10/text/original/epub/OEBPS/document_1/document_1.html#_Toc172118755"^^xsd:anyURI ;
    dcat:theme legcons:Item .

C2020A00012:630 a legcons:Item,
        owl:Class,
        dcat:Resource ;
    rdfs:label "Item - I630 407  Simplified outline of this Part"@en-AU ;
    dct:isPartOf C2020A00012:629 ;
    dct:isReferencedBy C2020A00012: ;
    rdfs:comment "407  Simplified outline of this Part - Abrievated Graph Key: I630"@en-AU ;
    skos:definition "407  Simplified outline of this Part"@en-AU ;
    skos:narrower C2020A00012:629 ;
    skos:prefLabel "Item I630"@en-AU ;
    dcat:accessURL <https://www.legislation.gov.au/C2020A00012/2024-07-10/2024-07-10/text/original/epub/OEBPS/document_1/document_1.html#_Toc172119322> ;
    dcat:landingPage "https://www.legislation.gov.au/C2020A00012/2024-07-10/2024-07-10/text/original/epub/OEBPS/document_1/document_1.html#_Toc172119322"^^xsd:anyURI ;
    dcat:theme legcons:Item .

C2020A00012:632 a legcons:Item,
        owl:Class,
        dcat:Resource ;
    rdfs:label "Item - I632 408  Requirements to retain records"@en-AU ;
    dct:isPartOf C2020A00012:631 ;
    dct:isReferencedBy C2020A00012: ;
    rdfs:comment "408  Requirements to retain records - Abrievated Graph Key: I632"@en-AU ;
    skos:definition "408  Requirements to retain records"@en-AU ;
    skos:narrower C2020A00012:631 ;
    skos:prefLabel "Item I632"@en-AU ;
    dcat:accessURL <https://www.legislation.gov.au/C2020A00012/2024-07-10/2024-07-10/text/original/epub/OEBPS/document_1/document_1.html#_Toc172119324> ;
    dcat:landingPage "https://www.legislation.gov.au/C2020A00012/2024-07-10/2024-07-10/text/original/epub/OEBPS/document_1/document_1.html#_Toc172119324"^^xsd:anyURI ;
    dcat:theme legcons:Item .

C2020A00012:635 a legcons:Item,
        owl:Class,
        dcat:Resource ;
    rdfs:label "Item - I635 409  Simplified outline of this Part"@en-AU ;
    dct:isPartOf C2020A00012:634 ;
    dct:isReferencedBy C2020A00012: ;
    rdfs:comment "409  Simplified outline of this Part - Abrievated Graph Key: I635"@en-AU ;
    skos:definition "409  Simplified outline of this Part"@en-AU ;
    skos:narrower C2020A00012:634 ;
    skos:prefLabel "Item I635"@en-AU ;
    dcat:accessURL <https://www.legislation.gov.au/C2020A00012/2024-07-10/2024-07-10/text/original/epub/OEBPS/document_1/document_1.html#_Toc172119327> ;
    dcat:landingPage "https://www.legislation.gov.au/C2020A00012/2024-07-10/2024-07-10/text/original/epub/OEBPS/document_1/document_1.html#_Toc172119327"^^xsd:anyURI ;
    dcat:theme legcons:Item .

C2020A00012:637 a legcons:Item,
        owl:Class,
        dcat:Resource ;
    rdfs:label "Item - I637 410  Methods for taking testing and analysing certain samples"@en-AU ;
    dct:isPartOf C2020A00012:636 ;
    dct:isReferencedBy C2020A00012: ;
    rdfs:comment "410  Methods for taking testing and analysing certain samples - Abrievated Graph Key: I637"@en-AU ;
    skos:definition "410  Methods for taking testing and analysing certain samples"@en-AU ;
    skos:narrower C2020A00012:636 ;
    skos:prefLabel "Item I637"@en-AU ;
    dcat:accessURL <https://www.legislation.gov.au/C2020A00012/2024-07-10/2024-07-10/text/original/epub/OEBPS/document_1/document_1.html#_Toc172119329> ;
    dcat:landingPage "https://www.legislation.gov.au/C2020A00012/2024-07-10/2024-07-10/text/original/epub/OEBPS/document_1/document_1.html#_Toc172119329"^^xsd:anyURI ;
    dcat:theme legcons:Item .

C2020A00012:638 a legcons:Item,
        owl:Class,
        dcat:Resource ;
    rdfs:label "Item - I638 411  Storage of samples"@en-AU ;
    dct:isPartOf C2020A00012:636 ;
    dct:isReferencedBy C2020A00012: ;
    rdfs:comment "411  Storage of samples - Abrievated Graph Key: I638"@en-AU ;
    skos:definition "411  Storage of samples"@en-AU ;
    skos:narrower C2020A00012:636 ;
    skos:prefLabel "Item I638"@en-AU ;
    dcat:accessURL <https://www.legislation.gov.au/C2020A00012/2024-07-10/2024-07-10/text/original/epub/OEBPS/document_1/document_1.html#_Toc172119330> ;
    dcat:landingPage "https://www.legislation.gov.au/C2020A00012/2024-07-10/2024-07-10/text/original/epub/OEBPS/document_1/document_1.html#_Toc172119330"^^xsd:anyURI ;
    dcat:theme legcons:Item .

C2020A00012:639 a legcons:Item,
        owl:Class,
        dcat:Resource ;
    rdfs:label "Item - I639 412  Test or analysis may result in destruction or reduction in value of sample"@en-AU ;
    dct:isPartOf C2020A00012:636 ;
    dct:isReferencedBy C2020A00012: ;
    rdfs:comment "412  Test or analysis may result in destruction or reduction in value of sample - Abrievated Graph Key: I639"@en-AU ;
    skos:definition "412  Test or analysis may result in destruction or reduction in value of sample"@en-AU ;
    skos:narrower C2020A00012:636 ;
    skos:prefLabel "Item I639"@en-AU ;
    dcat:accessURL <https://www.legislation.gov.au/C2020A00012/2024-07-10/2024-07-10/text/original/epub/OEBPS/document_1/document_1.html#_Toc172119331> ;
    dcat:landingPage "https://www.legislation.gov.au/C2020A00012/2024-07-10/2024-07-10/text/original/epub/OEBPS/document_1/document_1.html#_Toc172119331"^^xsd:anyURI ;
    dcat:theme legcons:Item .

C2020A00012:64 a legcons:Item,
        owl:Class,
        dcat:Resource ;
    rdfs:label "Item - I64 50  Making false or misleading representation about non prescribed goods that are entered for export"@en-AU ;
    dct:isPartOf C2020A00012:28 ;
    dct:isReferencedBy C2020A00012: ;
    rdfs:comment "50  Making false or misleading representation about non prescribed goods that are entered for export - Abrievated Graph Key: I64"@en-AU ;
    skos:definition "50  Making false or misleading representation about non prescribed goods that are entered for export"@en-AU ;
    skos:narrower C2020A00012:28 ;
    skos:prefLabel "Item I64"@en-AU ;
    dcat:accessURL <https://www.legislation.gov.au/C2020A00012/2024-07-10/2024-07-10/text/original/epub/OEBPS/document_1/document_1.html#_Toc172118756> ;
    dcat:landingPage "https://www.legislation.gov.au/C2020A00012/2024-07-10/2024-07-10/text/original/epub/OEBPS/document_1/document_1.html#_Toc172118756"^^xsd:anyURI ;
    dcat:theme legcons:Item .

C2020A00012:640 a legcons:Item,
        owl:Class,
        dcat:Resource ;
    rdfs:label "Item - I640 413  Appointment of analyst"@en-AU ;
    dct:isPartOf C2020A00012:636 ;
    dct:isReferencedBy C2020A00012: ;
    rdfs:comment "413  Appointment of analyst - Abrievated Graph Key: I640"@en-AU ;
    skos:definition "413  Appointment of analyst"@en-AU ;
    skos:narrower C2020A00012:636 ;
    skos:prefLabel "Item I640"@en-AU ;
    dcat:accessURL <https://www.legislation.gov.au/C2020A00012/2024-07-10/2024-07-10/text/original/epub/OEBPS/document_1/document_1.html#_Toc172119332> ;
    dcat:landingPage "https://www.legislation.gov.au/C2020A00012/2024-07-10/2024-07-10/text/original/epub/OEBPS/document_1/document_1.html#_Toc172119332"^^xsd:anyURI ;
    dcat:theme legcons:Item .

C2020A00012:641 a legcons:Item,
        owl:Class,
        dcat:Resource ;
    rdfs:label "Item - I641 414  Analyst may give certificate"@en-AU ;
    dct:isPartOf C2020A00012:636 ;
    dct:isReferencedBy C2020A00012: ;
    rdfs:comment "414  Analyst may give certificate - Abrievated Graph Key: I641"@en-AU ;
    skos:definition "414  Analyst may give certificate"@en-AU ;
    skos:narrower C2020A00012:636 ;
    skos:prefLabel "Item I641"@en-AU ;
    dcat:accessURL <https://www.legislation.gov.au/C2020A00012/2024-07-10/2024-07-10/text/original/epub/OEBPS/document_1/document_1.html#_Toc172119333> ;
    dcat:landingPage "https://www.legislation.gov.au/C2020A00012/2024-07-10/2024-07-10/text/original/epub/OEBPS/document_1/document_1.html#_Toc172119333"^^xsd:anyURI ;
    dcat:theme legcons:Item .

C2020A00012:642 a legcons:Item,
        owl:Class,
        dcat:Resource ;
    rdfs:label "Item - I642 415  Admission of analysts certificate in proceedings"@en-AU ;
    dct:isPartOf C2020A00012:636 ;
    dct:isReferencedBy C2020A00012: ;
    rdfs:comment "415  Admission of analysts certificate in proceedings - Abrievated Graph Key: I642"@en-AU ;
    skos:definition "415  Admission of analysts certificate in proceedings"@en-AU ;
    skos:narrower C2020A00012:636 ;
    skos:prefLabel "Item I642"@en-AU ;
    dcat:accessURL <https://www.legislation.gov.au/C2020A00012/2024-07-10/2024-07-10/text/original/epub/OEBPS/document_1/document_1.html#_Toc172119334> ;
    dcat:landingPage "https://www.legislation.gov.au/C2020A00012/2024-07-10/2024-07-10/text/original/epub/OEBPS/document_1/document_1.html#_Toc172119334"^^xsd:anyURI ;
    dcat:theme legcons:Item .

C2020A00012:644 a legcons:Item,
        owl:Class,
        dcat:Resource ;
    rdfs:label "Item - I644 416  Forfeiture of goods"@en-AU ;
    dct:isPartOf C2020A00012:643 ;
    dct:isReferencedBy C2020A00012: ;
    rdfs:comment "416  Forfeiture of goods - Abrievated Graph Key: I644"@en-AU ;
    skos:definition "416  Forfeiture of goods"@en-AU ;
    skos:narrower C2020A00012:643 ;
    skos:prefLabel "Item I644"@en-AU ;
    dcat:accessURL <https://www.legislation.gov.au/C2020A00012/2024-07-10/2024-07-10/text/original/epub/OEBPS/document_1/document_1.html#_Toc172119336> ;
    dcat:landingPage "https://www.legislation.gov.au/C2020A00012/2024-07-10/2024-07-10/text/original/epub/OEBPS/document_1/document_1.html#_Toc172119336"^^xsd:anyURI ;
    dcat:theme legcons:Item .

C2020A00012:646 a legcons:Item,
        owl:Class,
        dcat:Resource ;
    rdfs:label "Item - I646 417  Person complying with direction or request must not damage or destroy goods"@en-AU ;
    dct:isPartOf C2020A00012:645 ;
    dct:isReferencedBy C2020A00012: ;
    rdfs:comment "417  Person complying with direction or request must not damage or destroy goods - Abrievated Graph Key: I646"@en-AU ;
    skos:definition "417  Person complying with direction or request must not damage or destroy goods"@en-AU ;
    skos:narrower C2020A00012:645 ;
    skos:prefLabel "Item I646"@en-AU ;
    dcat:accessURL <https://www.legislation.gov.au/C2020A00012/2024-07-10/2024-07-10/text/original/epub/OEBPS/document_1/document_1.html#_Toc172119338> ;
    dcat:landingPage "https://www.legislation.gov.au/C2020A00012/2024-07-10/2024-07-10/text/original/epub/OEBPS/document_1/document_1.html#_Toc172119338"^^xsd:anyURI ;
    dcat:theme legcons:Item .

C2020A00012:647 a legcons:Item,
        owl:Class,
        dcat:Resource ;
    rdfs:label "Item - I647 418  Goods seized in certain circumstances may be destroyed"@en-AU ;
    dct:isPartOf C2020A00012:645 ;
    dct:isReferencedBy C2020A00012: ;
    rdfs:comment "418  Goods seized in certain circumstances may be destroyed - Abrievated Graph Key: I647"@en-AU ;
    skos:definition "418  Goods seized in certain circumstances may be destroyed"@en-AU ;
    skos:narrower C2020A00012:645 ;
    skos:prefLabel "Item I647"@en-AU ;
    dcat:accessURL <https://www.legislation.gov.au/C2020A00012/2024-07-10/2024-07-10/text/original/epub/OEBPS/document_1/document_1.html#_Toc172119339> ;
    dcat:landingPage "https://www.legislation.gov.au/C2020A00012/2024-07-10/2024-07-10/text/original/epub/OEBPS/document_1/document_1.html#_Toc172119339"^^xsd:anyURI ;
    dcat:theme legcons:Item .

C2020A00012:648 a legcons:Item,
        owl:Class,
        dcat:Resource ;
    rdfs:label "Item - I648 419  Compensation for damaged or destroyed goods"@en-AU ;
    dct:isPartOf C2020A00012:645 ;
    dct:isReferencedBy C2020A00012: ;
    rdfs:comment "419  Compensation for damaged or destroyed goods - Abrievated Graph Key: I648"@en-AU ;
    skos:definition "419  Compensation for damaged or destroyed goods"@en-AU ;
    skos:narrower C2020A00012:645 ;
    skos:prefLabel "Item I648"@en-AU ;
    dcat:accessURL <https://www.legislation.gov.au/C2020A00012/2024-07-10/2024-07-10/text/original/epub/OEBPS/document_1/document_1.html#_Toc172119340> ;
    dcat:landingPage "https://www.legislation.gov.au/C2020A00012/2024-07-10/2024-07-10/text/original/epub/OEBPS/document_1/document_1.html#_Toc172119340"^^xsd:anyURI ;
    dcat:theme legcons:Item .

C2020A00012:649 a legcons:Item,
        owl:Class,
        dcat:Resource ;
    rdfs:label "Item - I649 420  Claims for and amount of compensation"@en-AU ;
    dct:isPartOf C2020A00012:645 ;
    dct:isReferencedBy C2020A00012: ;
    rdfs:comment "420  Claims for and amount of compensation - Abrievated Graph Key: I649"@en-AU ;
    skos:definition "420  Claims for and amount of compensation"@en-AU ;
    skos:narrower C2020A00012:645 ;
    skos:prefLabel "Item I649"@en-AU ;
    dcat:accessURL <https://www.legislation.gov.au/C2020A00012/2024-07-10/2024-07-10/text/original/epub/OEBPS/document_1/document_1.html#_Toc172119341> ;
    dcat:landingPage "https://www.legislation.gov.au/C2020A00012/2024-07-10/2024-07-10/text/original/epub/OEBPS/document_1/document_1.html#_Toc172119341"^^xsd:anyURI ;
    dcat:theme legcons:Item .

C2020A00012:65 a legcons:Item,
        owl:Class,
        dcat:Resource ;
    rdfs:label "Item - I65 50 A  Penalties for certain contraventions by bodies corporate"@en-AU ;
    dct:isPartOf C2020A00012:28 ;
    dct:isReferencedBy C2020A00012: ;
    rdfs:comment "50 A  Penalties for certain contraventions by bodies corporate - Abrievated Graph Key: I65"@en-AU ;
    skos:definition "50 A  Penalties for certain contraventions by bodies corporate"@en-AU ;
    skos:narrower C2020A00012:28 ;
    skos:prefLabel "Item I65"@en-AU ;
    dcat:accessURL <https://www.legislation.gov.au/C2020A00012/2024-07-10/2024-07-10/text/original/epub/OEBPS/document_1/document_1.html#_Toc172118757> ;
    dcat:landingPage "https://www.legislation.gov.au/C2020A00012/2024-07-10/2024-07-10/text/original/epub/OEBPS/document_1/document_1.html#_Toc172118757"^^xsd:anyURI ;
    dcat:theme legcons:Item .

C2020A00012:651 a legcons:Item,
        owl:Class,
        dcat:Resource ;
    rdfs:label "Item - I651 421  Treatment of partnerships"@en-AU ;
    dct:isPartOf C2020A00012:650 ;
    dct:isReferencedBy C2020A00012: ;
    rdfs:comment "421  Treatment of partnerships - Abrievated Graph Key: I651"@en-AU ;
    skos:definition "421  Treatment of partnerships"@en-AU ;
    skos:narrower C2020A00012:650 ;
    skos:prefLabel "Item I651"@en-AU ;
    dcat:accessURL <https://www.legislation.gov.au/C2020A00012/2024-07-10/2024-07-10/text/original/epub/OEBPS/document_1/document_1.html#_Toc172119343> ;
    dcat:landingPage "https://www.legislation.gov.au/C2020A00012/2024-07-10/2024-07-10/text/original/epub/OEBPS/document_1/document_1.html#_Toc172119343"^^xsd:anyURI ;
    dcat:theme legcons:Item .

C2020A00012:652 a legcons:Item,
        owl:Class,
        dcat:Resource ;
    rdfs:label "Item - I652 422  Treatment of unincorporated associations"@en-AU ;
    dct:isPartOf C2020A00012:650 ;
    dct:isReferencedBy C2020A00012: ;
    rdfs:comment "422  Treatment of unincorporated associations - Abrievated Graph Key: I652"@en-AU ;
    skos:definition "422  Treatment of unincorporated associations"@en-AU ;
    skos:narrower C2020A00012:650 ;
    skos:prefLabel "Item I652"@en-AU ;
    dcat:accessURL <https://www.legislation.gov.au/C2020A00012/2024-07-10/2024-07-10/text/original/epub/OEBPS/document_1/document_1.html#_Toc172119344> ;
    dcat:landingPage "https://www.legislation.gov.au/C2020A00012/2024-07-10/2024-07-10/text/original/epub/OEBPS/document_1/document_1.html#_Toc172119344"^^xsd:anyURI ;
    dcat:theme legcons:Item .

C2020A00012:653 a legcons:Item,
        owl:Class,
        dcat:Resource ;
    rdfs:label "Item - I653 423  Treatment of trusts"@en-AU ;
    dct:isPartOf C2020A00012:650 ;
    dct:isReferencedBy C2020A00012: ;
    rdfs:comment "423  Treatment of trusts - Abrievated Graph Key: I653"@en-AU ;
    skos:definition "423  Treatment of trusts"@en-AU ;
    skos:narrower C2020A00012:650 ;
    skos:prefLabel "Item I653"@en-AU ;
    dcat:accessURL <https://www.legislation.gov.au/C2020A00012/2024-07-10/2024-07-10/text/original/epub/OEBPS/document_1/document_1.html#_Toc172119345> ;
    dcat:landingPage "https://www.legislation.gov.au/C2020A00012/2024-07-10/2024-07-10/text/original/epub/OEBPS/document_1/document_1.html#_Toc172119345"^^xsd:anyURI ;
    dcat:theme legcons:Item .

C2020A00012:655 a legcons:Item,
        owl:Class,
        dcat:Resource ;
    rdfs:label "Item - I655 424  Report to Parliament about export of livestock"@en-AU ;
    dct:isPartOf C2020A00012:654 ;
    dct:isReferencedBy C2020A00012: ;
    rdfs:comment "424  Report to Parliament about export of livestock - Abrievated Graph Key: I655"@en-AU ;
    skos:definition "424  Report to Parliament about export of livestock"@en-AU ;
    skos:narrower C2020A00012:654 ;
    skos:prefLabel "Item I655"@en-AU ;
    dcat:accessURL <https://www.legislation.gov.au/C2020A00012/2024-07-10/2024-07-10/text/original/epub/OEBPS/document_1/document_1.html#_Toc172119347> ;
    dcat:landingPage "https://www.legislation.gov.au/C2020A00012/2024-07-10/2024-07-10/text/original/epub/OEBPS/document_1/document_1.html#_Toc172119347"^^xsd:anyURI ;
    dcat:theme legcons:Item .

C2020A00012:658 a legcons:Item,
        owl:Class,
        dcat:Resource ;
    rdfs:label "Item - I658 424 A  Arrangements and grants in relation to the phasing out of the export of live sheep by sea"@en-AU ;
    dct:isPartOf C2020A00012:657 ;
    dct:isReferencedBy C2020A00012: ;
    rdfs:comment "424 A  Arrangements and grants in relation to the phasing out of the export of live sheep by sea - Abrievated Graph Key: I658"@en-AU ;
    skos:definition "424 A  Arrangements and grants in relation to the phasing out of the export of live sheep by sea"@en-AU ;
    skos:narrower C2020A00012:657 ;
    skos:prefLabel "Item I658"@en-AU ;
    dcat:accessURL <https://www.legislation.gov.au/C2020A00012/2024-07-10/2024-07-10/text/original/epub/OEBPS/document_1/document_1.html#_Toc172119350> ;
    dcat:landingPage "https://www.legislation.gov.au/C2020A00012/2024-07-10/2024-07-10/text/original/epub/OEBPS/document_1/document_1.html#_Toc172119350"^^xsd:anyURI ;
    dcat:theme legcons:Item .

C2020A00012:659 a legcons:Item,
        owl:Class,
        dcat:Resource ;
    rdfs:label "Item - I659 424 B  Executive power of the Commonwealth"@en-AU ;
    dct:isPartOf C2020A00012:657 ;
    dct:isReferencedBy C2020A00012: ;
    rdfs:comment "424 B  Executive power of the Commonwealth - Abrievated Graph Key: I659"@en-AU ;
    skos:definition "424 B  Executive power of the Commonwealth"@en-AU ;
    skos:narrower C2020A00012:657 ;
    skos:prefLabel "Item I659"@en-AU ;
    dcat:accessURL <https://www.legislation.gov.au/C2020A00012/2024-07-10/2024-07-10/text/original/epub/OEBPS/document_1/document_1.html#_Toc172119351> ;
    dcat:landingPage "https://www.legislation.gov.au/C2020A00012/2024-07-10/2024-07-10/text/original/epub/OEBPS/document_1/document_1.html#_Toc172119351"^^xsd:anyURI ;
    dcat:theme legcons:Item .

C2020A00012:66 a legcons:Part,
        owl:Class,
        dcat:Resource ;
    rdfs:label "Part - P66 Part 2 Exemptions"@en-AU ;
    dct:isPartOf C2020A00012:27 ;
    dct:isReferencedBy C2020A00012: ;
    rdfs:comment "Part 2 Exemptions - Abrievated Graph Key: P66"@en-AU ;
    skos:definition "Part 2 Exemptions"@en-AU ;
    skos:narrower C2020A00012:27 ;
    skos:prefLabel "Part P66"@en-AU ;
    dcat:accessURL <https://www.legislation.gov.au/C2020A00012/2024-07-10/2024-07-10/text/original/epub/OEBPS/document_1/document_1.html#_Toc172118758> ;
    dcat:landingPage "https://www.legislation.gov.au/C2020A00012/2024-07-10/2024-07-10/text/original/epub/OEBPS/document_1/document_1.html#_Toc172118758"^^xsd:anyURI ;
    dcat:theme legcons:Part .

C2020A00012:660 a legcons:Item,
        owl:Class,
        dcat:Resource ;
    rdfs:label "Item - I660 424 C  Inclusion of information in annual reports"@en-AU ;
    dct:isPartOf C2020A00012:657 ;
    dct:isReferencedBy C2020A00012: ;
    rdfs:comment "424 C  Inclusion of information in annual reports - Abrievated Graph Key: I660"@en-AU ;
    skos:definition "424 C  Inclusion of information in annual reports"@en-AU ;
    skos:narrower C2020A00012:657 ;
    skos:prefLabel "Item I660"@en-AU ;
    dcat:accessURL <https://www.legislation.gov.au/C2020A00012/2024-07-10/2024-07-10/text/original/epub/OEBPS/document_1/document_1.html#_Toc172119352> ;
    dcat:landingPage "https://www.legislation.gov.au/C2020A00012/2024-07-10/2024-07-10/text/original/epub/OEBPS/document_1/document_1.html#_Toc172119352"^^xsd:anyURI ;
    dcat:theme legcons:Item .

C2020A00012:661 a legcons:Item,
        owl:Class,
        dcat:Resource ;
    rdfs:label "Item - I661 424 D  Delegation"@en-AU ;
    dct:isPartOf C2020A00012:657 ;
    dct:isReferencedBy C2020A00012: ;
    rdfs:comment "424 D  Delegation - Abrievated Graph Key: I661"@en-AU ;
    skos:definition "424 D  Delegation"@en-AU ;
    skos:narrower C2020A00012:657 ;
    skos:prefLabel "Item I661"@en-AU ;
    dcat:accessURL <https://www.legislation.gov.au/C2020A00012/2024-07-10/2024-07-10/text/original/epub/OEBPS/document_1/document_1.html#_Toc172119353> ;
    dcat:landingPage "https://www.legislation.gov.au/C2020A00012/2024-07-10/2024-07-10/text/original/epub/OEBPS/document_1/document_1.html#_Toc172119353"^^xsd:anyURI ;
    dcat:theme legcons:Item .

C2020A00012:663 a legcons:Item,
        owl:Class,
        dcat:Resource ;
    rdfs:label "Item - I663 424 E  Programs in relation to the phasing out of the export of live sheep by sea"@en-AU ;
    dct:isPartOf C2020A00012:662 ;
    dct:isReferencedBy C2020A00012: ;
    rdfs:comment "424 E  Programs in relation to the phasing out of the export of live sheep by sea - Abrievated Graph Key: I663"@en-AU ;
    skos:definition "424 E  Programs in relation to the phasing out of the export of live sheep by sea"@en-AU ;
    skos:narrower C2020A00012:662 ;
    skos:prefLabel "Item I663"@en-AU ;
    dcat:accessURL <https://www.legislation.gov.au/C2020A00012/2024-07-10/2024-07-10/text/original/epub/OEBPS/document_1/document_1.html#_Toc172119355> ;
    dcat:landingPage "https://www.legislation.gov.au/C2020A00012/2024-07-10/2024-07-10/text/original/epub/OEBPS/document_1/document_1.html#_Toc172119355"^^xsd:anyURI ;
    dcat:theme legcons:Item .

C2020A00012:664 a legcons:Item,
        owl:Class,
        dcat:Resource ;
    rdfs:label "Item - I664 424 F  Arrangements in relation to prescribed programs"@en-AU ;
    dct:isPartOf C2020A00012:662 ;
    dct:isReferencedBy C2020A00012: ;
    rdfs:comment "424 F  Arrangements in relation to prescribed programs - Abrievated Graph Key: I664"@en-AU ;
    skos:definition "424 F  Arrangements in relation to prescribed programs"@en-AU ;
    skos:narrower C2020A00012:662 ;
    skos:prefLabel "Item I664"@en-AU ;
    dcat:accessURL <https://www.legislation.gov.au/C2020A00012/2024-07-10/2024-07-10/text/original/epub/OEBPS/document_1/document_1.html#_Toc172119356> ;
    dcat:landingPage "https://www.legislation.gov.au/C2020A00012/2024-07-10/2024-07-10/text/original/epub/OEBPS/document_1/document_1.html#_Toc172119356"^^xsd:anyURI ;
    dcat:theme legcons:Item .

C2020A00012:665 a legcons:Item,
        owl:Class,
        dcat:Resource ;
    rdfs:label "Item - I665 424 G  Terms and conditions for arrangements in relation to prescribed programs"@en-AU ;
    dct:isPartOf C2020A00012:662 ;
    dct:isReferencedBy C2020A00012: ;
    rdfs:comment "424 G  Terms and conditions for arrangements in relation to prescribed programs - Abrievated Graph Key: I665"@en-AU ;
    skos:definition "424 G  Terms and conditions for arrangements in relation to prescribed programs"@en-AU ;
    skos:narrower C2020A00012:662 ;
    skos:prefLabel "Item I665"@en-AU ;
    dcat:accessURL <https://www.legislation.gov.au/C2020A00012/2024-07-10/2024-07-10/text/original/epub/OEBPS/document_1/document_1.html#_Toc172119357> ;
    dcat:landingPage "https://www.legislation.gov.au/C2020A00012/2024-07-10/2024-07-10/text/original/epub/OEBPS/document_1/document_1.html#_Toc172119357"^^xsd:anyURI ;
    dcat:theme legcons:Item .

C2020A00012:666 a legcons:Item,
        owl:Class,
        dcat:Resource ;
    rdfs:label "Item - I666 424 H  Delegation"@en-AU ;
    dct:isPartOf C2020A00012:662 ;
    dct:isReferencedBy C2020A00012: ;
    rdfs:comment "424 H  Delegation - Abrievated Graph Key: I666"@en-AU ;
    skos:definition "424 H  Delegation"@en-AU ;
    skos:narrower C2020A00012:662 ;
    skos:prefLabel "Item I666"@en-AU ;
    dcat:accessURL <https://www.legislation.gov.au/C2020A00012/2024-07-10/2024-07-10/text/original/epub/OEBPS/document_1/document_1.html#_Toc172119358> ;
    dcat:landingPage "https://www.legislation.gov.au/C2020A00012/2024-07-10/2024-07-10/text/original/epub/OEBPS/document_1/document_1.html#_Toc172119358"^^xsd:anyURI ;
    dcat:theme legcons:Item .

C2020A00012:667 a legcons:Item,
        owl:Class,
        dcat:Resource ;
    rdfs:label "Item - I667 424 J  Inclusion of information in annual reports"@en-AU ;
    dct:isPartOf C2020A00012:662 ;
    dct:isReferencedBy C2020A00012: ;
    rdfs:comment "424 J  Inclusion of information in annual reports - Abrievated Graph Key: I667"@en-AU ;
    skos:definition "424 J  Inclusion of information in annual reports"@en-AU ;
    skos:narrower C2020A00012:662 ;
    skos:prefLabel "Item I667"@en-AU ;
    dcat:accessURL <https://www.legislation.gov.au/C2020A00012/2024-07-10/2024-07-10/text/original/epub/OEBPS/document_1/document_1.html#_Toc172119359> ;
    dcat:landingPage "https://www.legislation.gov.au/C2020A00012/2024-07-10/2024-07-10/text/original/epub/OEBPS/document_1/document_1.html#_Toc172119359"^^xsd:anyURI ;
    dcat:theme legcons:Item .

C2020A00012:668 a legcons:Item,
        owl:Class,
        dcat:Resource ;
    rdfs:label "Item - I668 424 K  Executive power of the Commonwealth"@en-AU ;
    dct:isPartOf C2020A00012:662 ;
    dct:isReferencedBy C2020A00012: ;
    rdfs:comment "424 K  Executive power of the Commonwealth - Abrievated Graph Key: I668"@en-AU ;
    skos:definition "424 K  Executive power of the Commonwealth"@en-AU ;
    skos:narrower C2020A00012:662 ;
    skos:prefLabel "Item I668"@en-AU ;
    dcat:accessURL <https://www.legislation.gov.au/C2020A00012/2024-07-10/2024-07-10/text/original/epub/OEBPS/document_1/document_1.html#_Toc172119360> ;
    dcat:landingPage "https://www.legislation.gov.au/C2020A00012/2024-07-10/2024-07-10/text/original/epub/OEBPS/document_1/document_1.html#_Toc172119360"^^xsd:anyURI ;
    dcat:theme legcons:Item .

C2020A00012:669 a legcons:Item,
        owl:Class,
        dcat:Resource ;
    rdfs:label "Item - I669 424 L  Relationship of this Subdivision with the Public Governance Performance and Accountability Act 2013"@en-AU ;
    dct:isPartOf C2020A00012:662 ;
    dct:isReferencedBy C2020A00012: ;
    rdfs:comment "424 L  Relationship of this Subdivision with the Public Governance Performance and Accountability Act 2013 - Abrievated Graph Key: I669"@en-AU ;
    skos:definition "424 L  Relationship of this Subdivision with the Public Governance Performance and Accountability Act 2013"@en-AU ;
    skos:narrower C2020A00012:662 ;
    skos:prefLabel "Item I669"@en-AU ;
    dcat:accessURL <https://www.legislation.gov.au/C2020A00012/2024-07-10/2024-07-10/text/original/epub/OEBPS/document_1/document_1.html#_Toc172119361> ;
    dcat:landingPage "https://www.legislation.gov.au/C2020A00012/2024-07-10/2024-07-10/text/original/epub/OEBPS/document_1/document_1.html#_Toc172119361"^^xsd:anyURI ;
    dcat:theme legcons:Item .

C2020A00012:671 a legcons:Item,
        owl:Class,
        dcat:Resource ;
    rdfs:label "Item - I671 425  Compensation for acquisition of property"@en-AU ;
    dct:isPartOf C2020A00012:670 ;
    dct:isReferencedBy C2020A00012: ;
    rdfs:comment "425  Compensation for acquisition of property - Abrievated Graph Key: I671"@en-AU ;
    skos:definition "425  Compensation for acquisition of property"@en-AU ;
    skos:narrower C2020A00012:670 ;
    skos:prefLabel "Item I671"@en-AU ;
    dcat:accessURL <https://www.legislation.gov.au/C2020A00012/2024-07-10/2024-07-10/text/original/epub/OEBPS/document_1/document_1.html#_Toc172119363> ;
    dcat:landingPage "https://www.legislation.gov.au/C2020A00012/2024-07-10/2024-07-10/text/original/epub/OEBPS/document_1/document_1.html#_Toc172119363"^^xsd:anyURI ;
    dcat:theme legcons:Item .

C2020A00012:672 a legcons:Item,
        owl:Class,
        dcat:Resource ;
    rdfs:label "Item - I672 426  Privilege against self incrimination"@en-AU ;
    dct:isPartOf C2020A00012:670 ;
    dct:isReferencedBy C2020A00012: ;
    rdfs:comment "426  Privilege against self incrimination - Abrievated Graph Key: I672"@en-AU ;
    skos:definition "426  Privilege against self incrimination"@en-AU ;
    skos:narrower C2020A00012:670 ;
    skos:prefLabel "Item I672"@en-AU ;
    dcat:accessURL <https://www.legislation.gov.au/C2020A00012/2024-07-10/2024-07-10/text/original/epub/OEBPS/document_1/document_1.html#_Toc172119364> ;
    dcat:landingPage "https://www.legislation.gov.au/C2020A00012/2024-07-10/2024-07-10/text/original/epub/OEBPS/document_1/document_1.html#_Toc172119364"^^xsd:anyURI ;
    dcat:theme legcons:Item .

C2020A00012:673 a legcons:Item,
        owl:Class,
        dcat:Resource ;
    rdfs:label "Item - I673 427  Hindering compliance with the Act etc"@en-AU ;
    dct:isPartOf C2020A00012:670 ;
    dct:isReferencedBy C2020A00012: ;
    rdfs:comment "427  Hindering compliance with the Act etc - Abrievated Graph Key: I673"@en-AU ;
    skos:definition "427  Hindering compliance with the Act etc"@en-AU ;
    skos:narrower C2020A00012:670 ;
    skos:prefLabel "Item I673"@en-AU ;
    dcat:accessURL <https://www.legislation.gov.au/C2020A00012/2024-07-10/2024-07-10/text/original/epub/OEBPS/document_1/document_1.html#_Toc172119365> ;
    dcat:landingPage "https://www.legislation.gov.au/C2020A00012/2024-07-10/2024-07-10/text/original/epub/OEBPS/document_1/document_1.html#_Toc172119365"^^xsd:anyURI ;
    dcat:theme legcons:Item .

C2020A00012:674 a legcons:Item,
        owl:Class,
        dcat:Resource ;
    rdfs:label "Item - I674 427 A  Influencing a person performing functions or duties or exercising powers"@en-AU ;
    dct:isPartOf C2020A00012:670 ;
    dct:isReferencedBy C2020A00012: ;
    rdfs:comment "427 A  Influencing a person performing functions or duties or exercising powers - Abrievated Graph Key: I674"@en-AU ;
    skos:definition "427 A  Influencing a person performing functions or duties or exercising powers"@en-AU ;
    skos:narrower C2020A00012:670 ;
    skos:prefLabel "Item I674"@en-AU ;
    dcat:accessURL <https://www.legislation.gov.au/C2020A00012/2024-07-10/2024-07-10/text/original/epub/OEBPS/document_1/document_1.html#_Toc172119366> ;
    dcat:landingPage "https://www.legislation.gov.au/C2020A00012/2024-07-10/2024-07-10/text/original/epub/OEBPS/document_1/document_1.html#_Toc172119366"^^xsd:anyURI ;
    dcat:theme legcons:Item .

C2020A00012:675 a legcons:Item,
        owl:Class,
        dcat:Resource ;
    rdfs:label "Item - I675 428  Power or requirement to do or cause a thing to be done"@en-AU ;
    dct:isPartOf C2020A00012:670 ;
    dct:isReferencedBy C2020A00012: ;
    rdfs:comment "428  Power or requirement to do or cause a thing to be done - Abrievated Graph Key: I675"@en-AU ;
    skos:definition "428  Power or requirement to do or cause a thing to be done"@en-AU ;
    skos:narrower C2020A00012:670 ;
    skos:prefLabel "Item I675"@en-AU ;
    dcat:accessURL <https://www.legislation.gov.au/C2020A00012/2024-07-10/2024-07-10/text/original/epub/OEBPS/document_1/document_1.html#_Toc172119367> ;
    dcat:landingPage "https://www.legislation.gov.au/C2020A00012/2024-07-10/2024-07-10/text/original/epub/OEBPS/document_1/document_1.html#_Toc172119367"^^xsd:anyURI ;
    dcat:theme legcons:Item .

C2020A00012:676 a legcons:Item,
        owl:Class,
        dcat:Resource ;
    rdfs:label "Item - I676 429  Arrangements with States and Territories to assist in carrying out this Act"@en-AU ;
    dct:isPartOf C2020A00012:670 ;
    dct:isReferencedBy C2020A00012: ;
    rdfs:comment "429  Arrangements with States and Territories to assist in carrying out this Act - Abrievated Graph Key: I676"@en-AU ;
    skos:definition "429  Arrangements with States and Territories to assist in carrying out this Act"@en-AU ;
    skos:narrower C2020A00012:670 ;
    skos:prefLabel "Item I676"@en-AU ;
    dcat:accessURL <https://www.legislation.gov.au/C2020A00012/2024-07-10/2024-07-10/text/original/epub/OEBPS/document_1/document_1.html#_Toc172119368> ;
    dcat:landingPage "https://www.legislation.gov.au/C2020A00012/2024-07-10/2024-07-10/text/original/epub/OEBPS/document_1/document_1.html#_Toc172119368"^^xsd:anyURI ;
    dcat:theme legcons:Item .

C2020A00012:677 a legcons:Item,
        owl:Class,
        dcat:Resource ;
    rdfs:label "Item - I677 430  Protection from civil proceedings"@en-AU ;
    dct:isPartOf C2020A00012:670 ;
    dct:isReferencedBy C2020A00012: ;
    rdfs:comment "430  Protection from civil proceedings - Abrievated Graph Key: I677"@en-AU ;
    skos:definition "430  Protection from civil proceedings"@en-AU ;
    skos:narrower C2020A00012:670 ;
    skos:prefLabel "Item I677"@en-AU ;
    dcat:accessURL <https://www.legislation.gov.au/C2020A00012/2024-07-10/2024-07-10/text/original/epub/OEBPS/document_1/document_1.html#_Toc172119369> ;
    dcat:landingPage "https://www.legislation.gov.au/C2020A00012/2024-07-10/2024-07-10/text/original/epub/OEBPS/document_1/document_1.html#_Toc172119369"^^xsd:anyURI ;
    dcat:theme legcons:Item .

C2020A00012:678 a legcons:Item,
        owl:Class,
        dcat:Resource ;
    rdfs:label "Item - I678 431  Circumstances in which relevant Commonwealth liability of a person is taken to have been paid"@en-AU ;
    dct:isPartOf C2020A00012:670 ;
    dct:isReferencedBy C2020A00012: ;
    rdfs:comment "431  Circumstances in which relevant Commonwealth liability of a person is taken to have been paid - Abrievated Graph Key: I678"@en-AU ;
    skos:definition "431  Circumstances in which relevant Commonwealth liability of a person is taken to have been paid"@en-AU ;
    skos:narrower C2020A00012:670 ;
    skos:prefLabel "Item I678"@en-AU ;
    dcat:accessURL <https://www.legislation.gov.au/C2020A00012/2024-07-10/2024-07-10/text/original/epub/OEBPS/document_1/document_1.html#_Toc172119370> ;
    dcat:landingPage "https://www.legislation.gov.au/C2020A00012/2024-07-10/2024-07-10/text/original/epub/OEBPS/document_1/document_1.html#_Toc172119370"^^xsd:anyURI ;
    dcat:theme legcons:Item .

C2020A00012:679 a legcons:Item,
        owl:Class,
        dcat:Resource ;
    rdfs:label "Item - I679 432  Rules"@en-AU ;
    dct:isPartOf C2020A00012:670 ;
    dct:isReferencedBy C2020A00012: ;
    rdfs:comment "432  Rules - Abrievated Graph Key: I679"@en-AU ;
    skos:definition "432  Rules"@en-AU ;
    skos:narrower C2020A00012:670 ;
    skos:prefLabel "Item I679"@en-AU ;
    dcat:accessURL <https://www.legislation.gov.au/C2020A00012/2024-07-10/2024-07-10/text/original/epub/OEBPS/document_1/document_1.html#_Toc172119371> ;
    dcat:landingPage "https://www.legislation.gov.au/C2020A00012/2024-07-10/2024-07-10/text/original/epub/OEBPS/document_1/document_1.html#_Toc172119371"^^xsd:anyURI ;
    dcat:theme legcons:Item .

C2020A00012:68 a legcons:Item,
        owl:Class,
        dcat:Resource ;
    rdfs:label "Item - I68 51  Simplified outline of this Part"@en-AU ;
    dct:isPartOf C2020A00012:67 ;
    dct:isReferencedBy C2020A00012: ;
    rdfs:comment "51  Simplified outline of this Part - Abrievated Graph Key: I68"@en-AU ;
    skos:definition "51  Simplified outline of this Part"@en-AU ;
    skos:narrower C2020A00012:67 ;
    skos:prefLabel "Item I68"@en-AU ;
    dcat:accessURL <https://www.legislation.gov.au/C2020A00012/2024-07-10/2024-07-10/text/original/epub/OEBPS/document_1/document_1.html#_Toc172118760> ;
    dcat:landingPage "https://www.legislation.gov.au/C2020A00012/2024-07-10/2024-07-10/text/original/epub/OEBPS/document_1/document_1.html#_Toc172118760"^^xsd:anyURI ;
    dcat:theme legcons:Item .

C2020A00012:681 a legcons:Item,
        owl:Class,
        dcat:Resource ;
    rdfs:label "Item - I681 Endnote 1 About the endnotes"@en-AU ;
    dct:isPartOf C2020A00012:680 ;
    dct:isReferencedBy C2020A00012: ;
    rdfs:comment "Endnote 1 About the endnotes - Abrievated Graph Key: I681"@en-AU ;
    skos:definition "Endnote 1 About the endnotes"@en-AU ;
    skos:narrower C2020A00012:680 ;
    skos:prefLabel "Item I681"@en-AU ;
    dcat:accessURL <https://www.legislation.gov.au/C2020A00012/2024-07-10/2024-07-10/text/original/epub/OEBPS/document_1/document_1.html#_Toc172119373> ;
    dcat:landingPage "https://www.legislation.gov.au/C2020A00012/2024-07-10/2024-07-10/text/original/epub/OEBPS/document_1/document_1.html#_Toc172119373"^^xsd:anyURI ;
    dcat:theme legcons:Item .

C2020A00012:682 a legcons:Item,
        owl:Class,
        dcat:Resource ;
    rdfs:label "Item - I682 Endnote 2 Abbreviation key"@en-AU ;
    dct:isPartOf C2020A00012:680 ;
    dct:isReferencedBy C2020A00012: ;
    rdfs:comment "Endnote 2 Abbreviation key - Abrievated Graph Key: I682"@en-AU ;
    skos:definition "Endnote 2 Abbreviation key"@en-AU ;
    skos:narrower C2020A00012:680 ;
    skos:prefLabel "Item I682"@en-AU ;
    dcat:accessURL <https://www.legislation.gov.au/C2020A00012/2024-07-10/2024-07-10/text/original/epub/OEBPS/document_1/document_1.html#_Toc172119374> ;
    dcat:landingPage "https://www.legislation.gov.au/C2020A00012/2024-07-10/2024-07-10/text/original/epub/OEBPS/document_1/document_1.html#_Toc172119374"^^xsd:anyURI ;
    dcat:theme legcons:Item .

C2020A00012:683 a legcons:Item,
        owl:Class,
        dcat:Resource ;
    rdfs:label "Item - I683 Endnote 3 Legislation history"@en-AU ;
    dct:isPartOf C2020A00012:680 ;
    dct:isReferencedBy C2020A00012: ;
    rdfs:comment "Endnote 3 Legislation history - Abrievated Graph Key: I683"@en-AU ;
    skos:definition "Endnote 3 Legislation history"@en-AU ;
    skos:narrower C2020A00012:680 ;
    skos:prefLabel "Item I683"@en-AU ;
    dcat:accessURL <https://www.legislation.gov.au/C2020A00012/2024-07-10/2024-07-10/text/original/epub/OEBPS/document_1/document_1.html#_Toc172119375> ;
    dcat:landingPage "https://www.legislation.gov.au/C2020A00012/2024-07-10/2024-07-10/text/original/epub/OEBPS/document_1/document_1.html#_Toc172119375"^^xsd:anyURI ;
    dcat:theme legcons:Item .

C2020A00012:684 a legcons:Item,
        owl:Class,
        dcat:Resource ;
    rdfs:label "Item - I684 Endnote 4 Amendment history"@en-AU ;
    dct:isPartOf C2020A00012:680 ;
    dct:isReferencedBy C2020A00012: ;
    rdfs:comment "Endnote 4 Amendment history - Abrievated Graph Key: I684"@en-AU ;
    skos:definition "Endnote 4 Amendment history"@en-AU ;
    skos:narrower C2020A00012:680 ;
    skos:prefLabel "Item I684"@en-AU ;
    dcat:accessURL <https://www.legislation.gov.au/C2020A00012/2024-07-10/2024-07-10/text/original/epub/OEBPS/document_1/document_1.html#_Toc172119376> ;
    dcat:landingPage "https://www.legislation.gov.au/C2020A00012/2024-07-10/2024-07-10/text/original/epub/OEBPS/document_1/document_1.html#_Toc172119376"^^xsd:anyURI ;
    dcat:theme legcons:Item .

C2020A00012:69 a legcons:Item,
        owl:Class,
        dcat:Resource ;
    rdfs:label "Item - I69 52  Application of this Part"@en-AU ;
    dct:isPartOf C2020A00012:67 ;
    dct:isReferencedBy C2020A00012: ;
    rdfs:comment "52  Application of this Part - Abrievated Graph Key: I69"@en-AU ;
    skos:definition "52  Application of this Part"@en-AU ;
    skos:narrower C2020A00012:67 ;
    skos:prefLabel "Item I69"@en-AU ;
    dcat:accessURL <https://www.legislation.gov.au/C2020A00012/2024-07-10/2024-07-10/text/original/epub/OEBPS/document_1/document_1.html#_Toc172118761> ;
    dcat:landingPage "https://www.legislation.gov.au/C2020A00012/2024-07-10/2024-07-10/text/original/epub/OEBPS/document_1/document_1.html#_Toc172118761"^^xsd:anyURI ;
    dcat:theme legcons:Item .

C2020A00012:7 a legcons:Item,
        owl:Class,
        dcat:Resource ;
    rdfs:label "Item - I7 5  Act binds the Crown"@en-AU ;
    dct:isPartOf C2020A00012:1 ;
    dct:isReferencedBy C2020A00012: ;
    rdfs:comment "5  Act binds the Crown - Abrievated Graph Key: I7"@en-AU ;
    skos:definition "5  Act binds the Crown"@en-AU ;
    skos:narrower C2020A00012:1 ;
    skos:prefLabel "Item I7"@en-AU ;
    dcat:accessURL <https://www.legislation.gov.au/C2020A00012/2024-07-10/2024-07-10/text/original/epub/OEBPS/document_1/document_1.html#_Toc172118699> ;
    dcat:landingPage "https://www.legislation.gov.au/C2020A00012/2024-07-10/2024-07-10/text/original/epub/OEBPS/document_1/document_1.html#_Toc172118699"^^xsd:anyURI ;
    dcat:theme legcons:Item .

C2020A00012:71 a legcons:Item,
        owl:Class,
        dcat:Resource ;
    rdfs:label "Item - I71 53  Application for exemption"@en-AU ;
    dct:isPartOf C2020A00012:70 ;
    dct:isReferencedBy C2020A00012: ;
    rdfs:comment "53  Application for exemption - Abrievated Graph Key: I71"@en-AU ;
    skos:definition "53  Application for exemption"@en-AU ;
    skos:narrower C2020A00012:70 ;
    skos:prefLabel "Item I71"@en-AU ;
    dcat:accessURL <https://www.legislation.gov.au/C2020A00012/2024-07-10/2024-07-10/text/original/epub/OEBPS/document_1/document_1.html#_Toc172118763> ;
    dcat:landingPage "https://www.legislation.gov.au/C2020A00012/2024-07-10/2024-07-10/text/original/epub/OEBPS/document_1/document_1.html#_Toc172118763"^^xsd:anyURI ;
    dcat:theme legcons:Item .

C2020A00012:72 a legcons:Item,
        owl:Class,
        dcat:Resource ;
    rdfs:label "Item - I72 54  Secretary must decide whether to grant exemption"@en-AU ;
    dct:isPartOf C2020A00012:70 ;
    dct:isReferencedBy C2020A00012: ;
    rdfs:comment "54  Secretary must decide whether to grant exemption - Abrievated Graph Key: I72"@en-AU ;
    skos:definition "54  Secretary must decide whether to grant exemption"@en-AU ;
    skos:narrower C2020A00012:70 ;
    skos:prefLabel "Item I72"@en-AU ;
    dcat:accessURL <https://www.legislation.gov.au/C2020A00012/2024-07-10/2024-07-10/text/original/epub/OEBPS/document_1/document_1.html#_Toc172118764> ;
    dcat:landingPage "https://www.legislation.gov.au/C2020A00012/2024-07-10/2024-07-10/text/original/epub/OEBPS/document_1/document_1.html#_Toc172118764"^^xsd:anyURI ;
    dcat:theme legcons:Item .

C2020A00012:73 a legcons:Item,
        owl:Class,
        dcat:Resource ;
    rdfs:label "Item - I73 55  Exemption may be granted subject to conditions"@en-AU ;
    dct:isPartOf C2020A00012:70 ;
    dct:isReferencedBy C2020A00012: ;
    rdfs:comment "55  Exemption may be granted subject to conditions - Abrievated Graph Key: I73"@en-AU ;
    skos:definition "55  Exemption may be granted subject to conditions"@en-AU ;
    skos:narrower C2020A00012:70 ;
    skos:prefLabel "Item I73"@en-AU ;
    dcat:accessURL <https://www.legislation.gov.au/C2020A00012/2024-07-10/2024-07-10/text/original/epub/OEBPS/document_1/document_1.html#_Toc172118765> ;
    dcat:landingPage "https://www.legislation.gov.au/C2020A00012/2024-07-10/2024-07-10/text/original/epub/OEBPS/document_1/document_1.html#_Toc172118765"^^xsd:anyURI ;
    dcat:theme legcons:Item .

C2020A00012:74 a legcons:Item,
        owl:Class,
        dcat:Resource ;
    rdfs:label "Item - I74 56  Notice of decision"@en-AU ;
    dct:isPartOf C2020A00012:70 ;
    dct:isReferencedBy C2020A00012: ;
    rdfs:comment "56  Notice of decision - Abrievated Graph Key: I74"@en-AU ;
    skos:definition "56  Notice of decision"@en-AU ;
    skos:narrower C2020A00012:70 ;
    skos:prefLabel "Item I74"@en-AU ;
    dcat:accessURL <https://www.legislation.gov.au/C2020A00012/2024-07-10/2024-07-10/text/original/epub/OEBPS/document_1/document_1.html#_Toc172118766> ;
    dcat:landingPage "https://www.legislation.gov.au/C2020A00012/2024-07-10/2024-07-10/text/original/epub/OEBPS/document_1/document_1.html#_Toc172118766"^^xsd:anyURI ;
    dcat:theme legcons:Item .

C2020A00012:75 a legcons:Item,
        owl:Class,
        dcat:Resource ;
    rdfs:label "Item - I75 57  Period of effect of exemption"@en-AU ;
    dct:isPartOf C2020A00012:70 ;
    dct:isReferencedBy C2020A00012: ;
    rdfs:comment "57  Period of effect of exemption - Abrievated Graph Key: I75"@en-AU ;
    skos:definition "57  Period of effect of exemption"@en-AU ;
    skos:narrower C2020A00012:70 ;
    skos:prefLabel "Item I75"@en-AU ;
    dcat:accessURL <https://www.legislation.gov.au/C2020A00012/2024-07-10/2024-07-10/text/original/epub/OEBPS/document_1/document_1.html#_Toc172118767> ;
    dcat:landingPage "https://www.legislation.gov.au/C2020A00012/2024-07-10/2024-07-10/text/original/epub/OEBPS/document_1/document_1.html#_Toc172118767"^^xsd:anyURI ;
    dcat:theme legcons:Item .

C2020A00012:76 a legcons:Item,
        owl:Class,
        dcat:Resource ;
    rdfs:label "Item - I76 58  Variation of conditions of exemption"@en-AU ;
    dct:isPartOf C2020A00012:70 ;
    dct:isReferencedBy C2020A00012: ;
    rdfs:comment "58  Variation of conditions of exemption - Abrievated Graph Key: I76"@en-AU ;
    skos:definition "58  Variation of conditions of exemption"@en-AU ;
    skos:narrower C2020A00012:70 ;
    skos:prefLabel "Item I76"@en-AU ;
    dcat:accessURL <https://www.legislation.gov.au/C2020A00012/2024-07-10/2024-07-10/text/original/epub/OEBPS/document_1/document_1.html#_Toc172118768> ;
    dcat:landingPage "https://www.legislation.gov.au/C2020A00012/2024-07-10/2024-07-10/text/original/epub/OEBPS/document_1/document_1.html#_Toc172118768"^^xsd:anyURI ;
    dcat:theme legcons:Item .

C2020A00012:77 a legcons:Item,
        owl:Class,
        dcat:Resource ;
    rdfs:label "Item - I77 59  Revocation of exemption"@en-AU ;
    dct:isPartOf C2020A00012:70 ;
    dct:isReferencedBy C2020A00012: ;
    rdfs:comment "59  Revocation of exemption - Abrievated Graph Key: I77"@en-AU ;
    skos:definition "59  Revocation of exemption"@en-AU ;
    skos:narrower C2020A00012:70 ;
    skos:prefLabel "Item I77"@en-AU ;
    dcat:accessURL <https://www.legislation.gov.au/C2020A00012/2024-07-10/2024-07-10/text/original/epub/OEBPS/document_1/document_1.html#_Toc172118769> ;
    dcat:landingPage "https://www.legislation.gov.au/C2020A00012/2024-07-10/2024-07-10/text/original/epub/OEBPS/document_1/document_1.html#_Toc172118769"^^xsd:anyURI ;
    dcat:theme legcons:Item .

C2020A00012:78 a legcons:Item,
        owl:Class,
        dcat:Resource ;
    rdfs:label "Item - I78 60  Effect of exemption"@en-AU ;
    dct:isPartOf C2020A00012:70 ;
    dct:isReferencedBy C2020A00012: ;
    rdfs:comment "60  Effect of exemption - Abrievated Graph Key: I78"@en-AU ;
    skos:definition "60  Effect of exemption"@en-AU ;
    skos:narrower C2020A00012:70 ;
    skos:prefLabel "Item I78"@en-AU ;
    dcat:accessURL <https://www.legislation.gov.au/C2020A00012/2024-07-10/2024-07-10/text/original/epub/OEBPS/document_1/document_1.html#_Toc172118770> ;
    dcat:landingPage "https://www.legislation.gov.au/C2020A00012/2024-07-10/2024-07-10/text/original/epub/OEBPS/document_1/document_1.html#_Toc172118770"^^xsd:anyURI ;
    dcat:theme legcons:Item .

C2020A00012:79 a legcons:Part,
        owl:Class,
        dcat:Resource ;
    rdfs:label "Part - P79 Part 3 Government certificates"@en-AU ;
    dct:isPartOf C2020A00012:27 ;
    dct:isReferencedBy C2020A00012: ;
    rdfs:comment "Part 3 Government certificates - Abrievated Graph Key: P79"@en-AU ;
    skos:definition "Part 3 Government certificates"@en-AU ;
    skos:narrower C2020A00012:27 ;
    skos:prefLabel "Part P79"@en-AU ;
    dcat:accessURL <https://www.legislation.gov.au/C2020A00012/2024-07-10/2024-07-10/text/original/epub/OEBPS/document_1/document_1.html#_Toc172118771> ;
    dcat:landingPage "https://www.legislation.gov.au/C2020A00012/2024-07-10/2024-07-10/text/original/epub/OEBPS/document_1/document_1.html#_Toc172118771"^^xsd:anyURI ;
    dcat:theme legcons:Part .

C2020A00012:8 a legcons:Item,
        owl:Class,
        dcat:Resource ;
    rdfs:label "Item - I8 6  Application of this Act in Australia"@en-AU ;
    dct:isPartOf C2020A00012:1 ;
    dct:isReferencedBy C2020A00012: ;
    rdfs:comment "6  Application of this Act in Australia - Abrievated Graph Key: I8"@en-AU ;
    skos:definition "6  Application of this Act in Australia"@en-AU ;
    skos:narrower C2020A00012:1 ;
    skos:prefLabel "Item I8"@en-AU ;
    dcat:accessURL <https://www.legislation.gov.au/C2020A00012/2024-07-10/2024-07-10/text/original/epub/OEBPS/document_1/document_1.html#_Toc172118700> ;
    dcat:landingPage "https://www.legislation.gov.au/C2020A00012/2024-07-10/2024-07-10/text/original/epub/OEBPS/document_1/document_1.html#_Toc172118700"^^xsd:anyURI ;
    dcat:theme legcons:Item .

C2020A00012:81 a legcons:Item,
        owl:Class,
        dcat:Resource ;
    rdfs:label "Item - I81 61  Simplified outline of this Part"@en-AU ;
    dct:isPartOf C2020A00012:80 ;
    dct:isReferencedBy C2020A00012: ;
    rdfs:comment "61  Simplified outline of this Part - Abrievated Graph Key: I81"@en-AU ;
    skos:definition "61  Simplified outline of this Part"@en-AU ;
    skos:narrower C2020A00012:80 ;
    skos:prefLabel "Item I81"@en-AU ;
    dcat:accessURL <https://www.legislation.gov.au/C2020A00012/2024-07-10/2024-07-10/text/original/epub/OEBPS/document_1/document_1.html#_Toc172118773> ;
    dcat:landingPage "https://www.legislation.gov.au/C2020A00012/2024-07-10/2024-07-10/text/original/epub/OEBPS/document_1/document_1.html#_Toc172118773"^^xsd:anyURI ;
    dcat:theme legcons:Item .

C2020A00012:83 a legcons:Item,
        owl:Class,
        dcat:Resource ;
    rdfs:label "Item - I83 62  Rules may make provision for and in relation to government certificates"@en-AU ;
    dct:isPartOf C2020A00012:82 ;
    dct:isReferencedBy C2020A00012: ;
    rdfs:comment "62  Rules may make provision for and in relation to government certificates - Abrievated Graph Key: I83"@en-AU ;
    skos:definition "62  Rules may make provision for and in relation to government certificates"@en-AU ;
    skos:narrower C2020A00012:82 ;
    skos:prefLabel "Item I83"@en-AU ;
    dcat:accessURL <https://www.legislation.gov.au/C2020A00012/2024-07-10/2024-07-10/text/original/epub/OEBPS/document_1/document_1.html#_Toc172118775> ;
    dcat:landingPage "https://www.legislation.gov.au/C2020A00012/2024-07-10/2024-07-10/text/original/epub/OEBPS/document_1/document_1.html#_Toc172118775"^^xsd:anyURI ;
    dcat:theme legcons:Item .

C2020A00012:84 a legcons:Item,
        owl:Class,
        dcat:Resource ;
    rdfs:label "Item - I84 63  Issuing bodies"@en-AU ;
    dct:isPartOf C2020A00012:82 ;
    dct:isReferencedBy C2020A00012: ;
    rdfs:comment "63  Issuing bodies - Abrievated Graph Key: I84"@en-AU ;
    skos:definition "63  Issuing bodies"@en-AU ;
    skos:narrower C2020A00012:82 ;
    skos:prefLabel "Item I84"@en-AU ;
    dcat:accessURL <https://www.legislation.gov.au/C2020A00012/2024-07-10/2024-07-10/text/original/epub/OEBPS/document_1/document_1.html#_Toc172118776> ;
    dcat:landingPage "https://www.legislation.gov.au/C2020A00012/2024-07-10/2024-07-10/text/original/epub/OEBPS/document_1/document_1.html#_Toc172118776"^^xsd:anyURI ;
    dcat:theme legcons:Item .

C2020A00012:85 a legcons:Item,
        owl:Class,
        dcat:Resource ;
    rdfs:label "Item - I85 64  Certain issuing bodies may charge fees"@en-AU ;
    dct:isPartOf C2020A00012:82 ;
    dct:isReferencedBy C2020A00012: ;
    rdfs:comment "64  Certain issuing bodies may charge fees - Abrievated Graph Key: I85"@en-AU ;
    skos:definition "64  Certain issuing bodies may charge fees"@en-AU ;
    skos:narrower C2020A00012:82 ;
    skos:prefLabel "Item I85"@en-AU ;
    dcat:accessURL <https://www.legislation.gov.au/C2020A00012/2024-07-10/2024-07-10/text/original/epub/OEBPS/document_1/document_1.html#_Toc172118777> ;
    dcat:landingPage "https://www.legislation.gov.au/C2020A00012/2024-07-10/2024-07-10/text/original/epub/OEBPS/document_1/document_1.html#_Toc172118777"^^xsd:anyURI ;
    dcat:theme legcons:Item .

C2020A00012:87 a legcons:Item,
        owl:Class,
        dcat:Resource ;
    rdfs:label "Item - I87 65  Application for government certificate"@en-AU ;
    dct:isPartOf C2020A00012:86 ;
    dct:isReferencedBy C2020A00012: ;
    rdfs:comment "65  Application for government certificate - Abrievated Graph Key: I87"@en-AU ;
    skos:definition "65  Application for government certificate"@en-AU ;
    skos:narrower C2020A00012:86 ;
    skos:prefLabel "Item I87"@en-AU ;
    dcat:accessURL <https://www.legislation.gov.au/C2020A00012/2024-07-10/2024-07-10/text/original/epub/OEBPS/document_1/document_1.html#_Toc172118779> ;
    dcat:landingPage "https://www.legislation.gov.au/C2020A00012/2024-07-10/2024-07-10/text/original/epub/OEBPS/document_1/document_1.html#_Toc172118779"^^xsd:anyURI ;
    dcat:theme legcons:Item .

C2020A00012:88 a legcons:Item,
        owl:Class,
        dcat:Resource ;
    rdfs:label "Item - I88 66  Additional or corrected information"@en-AU ;
    dct:isPartOf C2020A00012:86 ;
    dct:isReferencedBy C2020A00012: ;
    rdfs:comment "66  Additional or corrected information - Abrievated Graph Key: I88"@en-AU ;
    skos:definition "66  Additional or corrected information"@en-AU ;
    skos:narrower C2020A00012:86 ;
    skos:prefLabel "Item I88"@en-AU ;
    dcat:accessURL <https://www.legislation.gov.au/C2020A00012/2024-07-10/2024-07-10/text/original/epub/OEBPS/document_1/document_1.html#_Toc172118780> ;
    dcat:landingPage "https://www.legislation.gov.au/C2020A00012/2024-07-10/2024-07-10/text/original/epub/OEBPS/document_1/document_1.html#_Toc172118780"^^xsd:anyURI ;
    dcat:theme legcons:Item .

C2020A00012:89 a legcons:Item,
        owl:Class,
        dcat:Resource ;
    rdfs:label "Item - I89 67  Issuing body must decide whether to issue government certificate"@en-AU ;
    dct:isPartOf C2020A00012:86 ;
    dct:isReferencedBy C2020A00012: ;
    rdfs:comment "67  Issuing body must decide whether to issue government certificate - Abrievated Graph Key: I89"@en-AU ;
    skos:definition "67  Issuing body must decide whether to issue government certificate"@en-AU ;
    skos:narrower C2020A00012:86 ;
    skos:prefLabel "Item I89"@en-AU ;
    dcat:accessURL <https://www.legislation.gov.au/C2020A00012/2024-07-10/2024-07-10/text/original/epub/OEBPS/document_1/document_1.html#_Toc172118781> ;
    dcat:landingPage "https://www.legislation.gov.au/C2020A00012/2024-07-10/2024-07-10/text/original/epub/OEBPS/document_1/document_1.html#_Toc172118781"^^xsd:anyURI ;
    dcat:theme legcons:Item .

C2020A00012:9 a legcons:Item,
        owl:Class,
        dcat:Resource ;
    rdfs:label "Item - I9 7  Limited application of this Act outside Australia"@en-AU ;
    dct:isPartOf C2020A00012:1 ;
    dct:isReferencedBy C2020A00012: ;
    rdfs:comment "7  Limited application of this Act outside Australia - Abrievated Graph Key: I9"@en-AU ;
    skos:definition "7  Limited application of this Act outside Australia"@en-AU ;
    skos:narrower C2020A00012:1 ;
    skos:prefLabel "Item I9"@en-AU ;
    dcat:accessURL <https://www.legislation.gov.au/C2020A00012/2024-07-10/2024-07-10/text/original/epub/OEBPS/document_1/document_1.html#_Toc172118701> ;
    dcat:landingPage "https://www.legislation.gov.au/C2020A00012/2024-07-10/2024-07-10/text/original/epub/OEBPS/document_1/document_1.html#_Toc172118701"^^xsd:anyURI ;
    dcat:theme legcons:Item .

C2020A00012:90 a legcons:Item,
        owl:Class,
        dcat:Resource ;
    rdfs:label "Item - I90 68  Powers of Secretary in relation to application"@en-AU ;
    dct:isPartOf C2020A00012:86 ;
    dct:isReferencedBy C2020A00012: ;
    rdfs:comment "68  Powers of Secretary in relation to application - Abrievated Graph Key: I90"@en-AU ;
    skos:definition "68  Powers of Secretary in relation to application"@en-AU ;
    skos:narrower C2020A00012:86 ;
    skos:prefLabel "Item I90"@en-AU ;
    dcat:accessURL <https://www.legislation.gov.au/C2020A00012/2024-07-10/2024-07-10/text/original/epub/OEBPS/document_1/document_1.html#_Toc172118782> ;
    dcat:landingPage "https://www.legislation.gov.au/C2020A00012/2024-07-10/2024-07-10/text/original/epub/OEBPS/document_1/document_1.html#_Toc172118782"^^xsd:anyURI ;
    dcat:theme legcons:Item .

C2020A00012:91 a legcons:Item,
        owl:Class,
        dcat:Resource ;
    rdfs:label "Item - I91 69  Applications in relation to certain kinds of non prescribed goods"@en-AU ;
    dct:isPartOf C2020A00012:86 ;
    dct:isReferencedBy C2020A00012: ;
    rdfs:comment "69  Applications in relation to certain kinds of non prescribed goods - Abrievated Graph Key: I91"@en-AU ;
    skos:definition "69  Applications in relation to certain kinds of non prescribed goods"@en-AU ;
    skos:narrower C2020A00012:86 ;
    skos:prefLabel "Item I91"@en-AU ;
    dcat:accessURL <https://www.legislation.gov.au/C2020A00012/2024-07-10/2024-07-10/text/original/epub/OEBPS/document_1/document_1.html#_Toc172118783> ;
    dcat:landingPage "https://www.legislation.gov.au/C2020A00012/2024-07-10/2024-07-10/text/original/epub/OEBPS/document_1/document_1.html#_Toc172118783"^^xsd:anyURI ;
    dcat:theme legcons:Item .

C2020A00012:92 a legcons:Item,
        owl:Class,
        dcat:Resource ;
    rdfs:label "Item - I92 70  Government certificate for goods that are to be or that have been exported from certain external Territories"@en-AU ;
    dct:isPartOf C2020A00012:86 ;
    dct:isReferencedBy C2020A00012: ;
    rdfs:comment "70  Government certificate for goods that are to be or that have been exported from certain external Territories - Abrievated Graph Key: I92"@en-AU ;
    skos:definition "70  Government certificate for goods that are to be or that have been exported from certain external Territories"@en-AU ;
    skos:narrower C2020A00012:86 ;
    skos:prefLabel "Item I92"@en-AU ;
    dcat:accessURL <https://www.legislation.gov.au/C2020A00012/2024-07-10/2024-07-10/text/original/epub/OEBPS/document_1/document_1.html#_Toc172118784> ;
    dcat:landingPage "https://www.legislation.gov.au/C2020A00012/2024-07-10/2024-07-10/text/original/epub/OEBPS/document_1/document_1.html#_Toc172118784"^^xsd:anyURI ;
    dcat:theme legcons:Item .

C2020A00012:93 a legcons:Item,
        owl:Class,
        dcat:Resource ;
    rdfs:label "Item - I93 71  Manner of issuing government certificate"@en-AU ;
    dct:isPartOf C2020A00012:86 ;
    dct:isReferencedBy C2020A00012: ;
    rdfs:comment "71  Manner of issuing government certificate - Abrievated Graph Key: I93"@en-AU ;
    skos:definition "71  Manner of issuing government certificate"@en-AU ;
    skos:narrower C2020A00012:86 ;
    skos:prefLabel "Item I93"@en-AU ;
    dcat:accessURL <https://www.legislation.gov.au/C2020A00012/2024-07-10/2024-07-10/text/original/epub/OEBPS/document_1/document_1.html#_Toc172118785> ;
    dcat:landingPage "https://www.legislation.gov.au/C2020A00012/2024-07-10/2024-07-10/text/original/epub/OEBPS/document_1/document_1.html#_Toc172118785"^^xsd:anyURI ;
    dcat:theme legcons:Item .

C2020A00012:94 a legcons:Item,
        owl:Class,
        dcat:Resource ;
    rdfs:label "Item - I94 72  Period of effect of government certificate"@en-AU ;
    dct:isPartOf C2020A00012:86 ;
    dct:isReferencedBy C2020A00012: ;
    rdfs:comment "72  Period of effect of government certificate - Abrievated Graph Key: I94"@en-AU ;
    skos:definition "72  Period of effect of government certificate"@en-AU ;
    skos:narrower C2020A00012:86 ;
    skos:prefLabel "Item I94"@en-AU ;
    dcat:accessURL <https://www.legislation.gov.au/C2020A00012/2024-07-10/2024-07-10/text/original/epub/OEBPS/document_1/document_1.html#_Toc172118786> ;
    dcat:landingPage "https://www.legislation.gov.au/C2020A00012/2024-07-10/2024-07-10/text/original/epub/OEBPS/document_1/document_1.html#_Toc172118786"^^xsd:anyURI ;
    dcat:theme legcons:Item .

C2020A00012:96 a legcons:Item,
        owl:Class,
        dcat:Resource ;
    rdfs:label "Item - I96 73  Secretary may require assessment of goods"@en-AU ;
    dct:isPartOf C2020A00012:95 ;
    dct:isReferencedBy C2020A00012: ;
    rdfs:comment "73  Secretary may require assessment of goods - Abrievated Graph Key: I96"@en-AU ;
    skos:definition "73  Secretary may require assessment of goods"@en-AU ;
    skos:narrower C2020A00012:95 ;
    skos:prefLabel "Item I96"@en-AU ;
    dcat:accessURL <https://www.legislation.gov.au/C2020A00012/2024-07-10/2024-07-10/text/original/epub/OEBPS/document_1/document_1.html#_Toc172118788> ;
    dcat:landingPage "https://www.legislation.gov.au/C2020A00012/2024-07-10/2024-07-10/text/original/epub/OEBPS/document_1/document_1.html#_Toc172118788"^^xsd:anyURI ;
    dcat:theme legcons:Item .

C2020A00012:97 a legcons:Item,
        owl:Class,
        dcat:Resource ;
    rdfs:label "Item - I97 74  Additional or corrected information in relation to application for government certificate etc"@en-AU ;
    dct:isPartOf C2020A00012:95 ;
    dct:isReferencedBy C2020A00012: ;
    rdfs:comment "74  Additional or corrected information in relation to application for government certificate etc - Abrievated Graph Key: I97"@en-AU ;
    skos:definition "74  Additional or corrected information in relation to application for government certificate etc"@en-AU ;
    skos:narrower C2020A00012:95 ;
    skos:prefLabel "Item I97"@en-AU ;
    dcat:accessURL <https://www.legislation.gov.au/C2020A00012/2024-07-10/2024-07-10/text/original/epub/OEBPS/document_1/document_1.html#_Toc172118789> ;
    dcat:landingPage "https://www.legislation.gov.au/C2020A00012/2024-07-10/2024-07-10/text/original/epub/OEBPS/document_1/document_1.html#_Toc172118789"^^xsd:anyURI ;
    dcat:theme legcons:Item .

C2020A00012:98 a legcons:Item,
        owl:Class,
        dcat:Resource ;
    rdfs:label "Item - I98 75  Revocation of government certificate"@en-AU ;
    dct:isPartOf C2020A00012:95 ;
    dct:isReferencedBy C2020A00012: ;
    rdfs:comment "75  Revocation of government certificate - Abrievated Graph Key: I98"@en-AU ;
    skos:definition "75  Revocation of government certificate"@en-AU ;
    skos:narrower C2020A00012:95 ;
    skos:prefLabel "Item I98"@en-AU ;
    dcat:accessURL <https://www.legislation.gov.au/C2020A00012/2024-07-10/2024-07-10/text/original/epub/OEBPS/document_1/document_1.html#_Toc172118790> ;
    dcat:landingPage "https://www.legislation.gov.au/C2020A00012/2024-07-10/2024-07-10/text/original/epub/OEBPS/document_1/document_1.html#_Toc172118790"^^xsd:anyURI ;
    dcat:theme legcons:Item .

C2020A00012:99 a legcons:Item,
        owl:Class,
        dcat:Resource ;
    rdfs:label "Item - I99 76  Return of government certificate"@en-AU ;
    dct:isPartOf C2020A00012:95 ;
    dct:isReferencedBy C2020A00012: ;
    rdfs:comment "76  Return of government certificate - Abrievated Graph Key: I99"@en-AU ;
    skos:definition "76  Return of government certificate"@en-AU ;
    skos:narrower C2020A00012:95 ;
    skos:prefLabel "Item I99"@en-AU ;
    dcat:accessURL <https://www.legislation.gov.au/C2020A00012/2024-07-10/2024-07-10/text/original/epub/OEBPS/document_1/document_1.html#_Toc172118791> ;
    dcat:landingPage "https://www.legislation.gov.au/C2020A00012/2024-07-10/2024-07-10/text/original/epub/OEBPS/document_1/document_1.html#_Toc172118791"^^xsd:anyURI ;
    dcat:theme legcons:Item .

C2020A00012:101 a legcons:Part,
        owl:Class,
        dcat:Resource ;
    rdfs:label "Part - P101 Part 1 Introduction"@en-AU ;
    dct:hasPart C2020A00012:102 ;
    dct:isPartOf C2020A00012:100 ;
    dct:isReferencedBy C2020A00012: ;
    rdfs:comment "Part 1 Introduction - Abrievated Graph Key: P101"@en-AU ;
    skos:broader C2020A00012:102 ;
    skos:definition "Part 1 Introduction"@en-AU ;
    skos:narrower C2020A00012:100 ;
    skos:prefLabel "Part P101"@en-AU ;
    dcat:accessURL <https://www.legislation.gov.au/C2020A00012/2024-07-10/2024-07-10/text/original/epub/OEBPS/document_1/document_1.html#_Toc172118793> ;
    dcat:landingPage "https://www.legislation.gov.au/C2020A00012/2024-07-10/2024-07-10/text/original/epub/OEBPS/document_1/document_1.html#_Toc172118793"^^xsd:anyURI ;
    dcat:theme legcons:Part .

C2020A00012:136 a legcons:Division,
        owl:Class,
        dcat:Resource ;
    rdfs:label "Division - D136 Division 1 Revocation requested by manager"@en-AU ;
    dct:hasPart C2020A00012:137 ;
    dct:isPartOf C2020A00012:135 ;
    dct:isReferencedBy C2020A00012: ;
    rdfs:comment "Division 1 Revocation requested by manager - Abrievated Graph Key: D136"@en-AU ;
    skos:broader C2020A00012:137 ;
    skos:definition "Division 1 Revocation requested by manager"@en-AU ;
    skos:narrower C2020A00012:135 ;
    skos:prefLabel "Division D136"@en-AU ;
    dcat:accessURL <https://www.legislation.gov.au/C2020A00012/2024-07-10/2024-07-10/text/original/epub/OEBPS/document_1/document_1.html#_Toc172118828> ;
    dcat:landingPage "https://www.legislation.gov.au/C2020A00012/2024-07-10/2024-07-10/text/original/epub/OEBPS/document_1/document_1.html#_Toc172118828"^^xsd:anyURI ;
    dcat:theme legcons:Division .

C2020A00012:142 a legcons:Division,
        owl:Class,
        dcat:Resource ;
    rdfs:label "Division - D142 Division 3 Other provisions"@en-AU ;
    dct:hasPart C2020A00012:143 ;
    dct:isPartOf C2020A00012:135 ;
    dct:isReferencedBy C2020A00012: ;
    rdfs:comment "Division 3 Other provisions - Abrievated Graph Key: D142"@en-AU ;
    skos:broader C2020A00012:143 ;
    skos:definition "Division 3 Other provisions"@en-AU ;
    skos:narrower C2020A00012:135 ;
    skos:prefLabel "Division D142"@en-AU ;
    dcat:accessURL <https://www.legislation.gov.au/C2020A00012/2024-07-10/2024-07-10/text/original/epub/OEBPS/document_1/document_1.html#_Toc172118834> ;
    dcat:landingPage "https://www.legislation.gov.au/C2020A00012/2024-07-10/2024-07-10/text/original/epub/OEBPS/document_1/document_1.html#_Toc172118834"^^xsd:anyURI ;
    dcat:theme legcons:Division .

C2020A00012:150 a legcons:Part,
        owl:Class,
        dcat:Resource ;
    rdfs:label "Part - P150 Part 1 Introduction"@en-AU ;
    dct:hasPart C2020A00012:151 ;
    dct:isPartOf C2020A00012:149 ;
    dct:isReferencedBy C2020A00012: ;
    rdfs:comment "Part 1 Introduction - Abrievated Graph Key: P150"@en-AU ;
    skos:broader C2020A00012:151 ;
    skos:definition "Part 1 Introduction"@en-AU ;
    skos:narrower C2020A00012:149 ;
    skos:prefLabel "Part P150"@en-AU ;
    dcat:accessURL <https://www.legislation.gov.au/C2020A00012/2024-07-10/2024-07-10/text/original/epub/OEBPS/document_1/document_1.html#_Toc172118842> ;
    dcat:landingPage "https://www.legislation.gov.au/C2020A00012/2024-07-10/2024-07-10/text/original/epub/OEBPS/document_1/document_1.html#_Toc172118842"^^xsd:anyURI ;
    dcat:theme legcons:Part .

C2020A00012:189 a legcons:Division,
        owl:Class,
        dcat:Resource ;
    rdfs:label "Division - D189 Division 1 Revocation requested by occupier"@en-AU ;
    dct:hasPart C2020A00012:190 ;
    dct:isPartOf C2020A00012:188 ;
    dct:isReferencedBy C2020A00012: ;
    rdfs:comment "Division 1 Revocation requested by occupier - Abrievated Graph Key: D189"@en-AU ;
    skos:broader C2020A00012:190 ;
    skos:definition "Division 1 Revocation requested by occupier"@en-AU ;
    skos:narrower C2020A00012:188 ;
    skos:prefLabel "Division D189"@en-AU ;
    dcat:accessURL <https://www.legislation.gov.au/C2020A00012/2024-07-10/2024-07-10/text/original/epub/OEBPS/document_1/document_1.html#_Toc172118881> ;
    dcat:landingPage "https://www.legislation.gov.au/C2020A00012/2024-07-10/2024-07-10/text/original/epub/OEBPS/document_1/document_1.html#_Toc172118881"^^xsd:anyURI ;
    dcat:theme legcons:Division .

C2020A00012:204 a legcons:Part,
        owl:Class,
        dcat:Resource ;
    rdfs:label "Part - P204 Part 8 Other matters"@en-AU ;
    dct:hasPart C2020A00012:205 ;
    dct:isPartOf C2020A00012:149 ;
    dct:isReferencedBy C2020A00012: ;
    rdfs:comment "Part 8 Other matters - Abrievated Graph Key: P204"@en-AU ;
    skos:broader C2020A00012:205 ;
    skos:definition "Part 8 Other matters"@en-AU ;
    skos:narrower C2020A00012:149 ;
    skos:prefLabel "Part P204"@en-AU ;
    dcat:accessURL <https://www.legislation.gov.au/C2020A00012/2024-07-10/2024-07-10/text/original/epub/OEBPS/document_1/document_1.html#_Toc172118896> ;
    dcat:landingPage "https://www.legislation.gov.au/C2020A00012/2024-07-10/2024-07-10/text/original/epub/OEBPS/document_1/document_1.html#_Toc172118896"^^xsd:anyURI ;
    dcat:theme legcons:Part .

C2020A00012:207 a legcons:Part,
        owl:Class,
        dcat:Resource ;
    rdfs:label "Part - P207 Part 1 Introduction"@en-AU ;
    dct:hasPart C2020A00012:208 ;
    dct:isPartOf C2020A00012:206 ;
    dct:isReferencedBy C2020A00012: ;
    rdfs:comment "Part 1 Introduction - Abrievated Graph Key: P207"@en-AU ;
    skos:broader C2020A00012:208 ;
    skos:definition "Part 1 Introduction"@en-AU ;
    skos:narrower C2020A00012:206 ;
    skos:prefLabel "Part P207"@en-AU ;
    dcat:accessURL <https://www.legislation.gov.au/C2020A00012/2024-07-10/2024-07-10/text/original/epub/OEBPS/document_1/document_1.html#_Toc172118899> ;
    dcat:landingPage "https://www.legislation.gov.au/C2020A00012/2024-07-10/2024-07-10/text/original/epub/OEBPS/document_1/document_1.html#_Toc172118899"^^xsd:anyURI ;
    dcat:theme legcons:Part .

C2020A00012:229 a legcons:Subdivision,
        owl:Class,
        dcat:Resource ;
    rdfs:label "Subdivision - S229 Subdivision CMatters relating to whether proposed variation of approved arrangement is significant"@en-AU ;
    dct:hasPart C2020A00012:230 ;
    dct:isPartOf C2020A00012:221 ;
    dct:isReferencedBy C2020A00012: ;
    rdfs:comment "Subdivision CMatters relating to whether proposed variation of approved arrangement is significant - Abrievated Graph Key: S229"@en-AU ;
    skos:broader C2020A00012:230 ;
    skos:definition "Subdivision CMatters relating to whether proposed variation of approved arrangement is significant"@en-AU ;
    skos:narrower C2020A00012:221 ;
    skos:prefLabel "Subdivision S229"@en-AU ;
    dcat:accessURL <https://www.legislation.gov.au/C2020A00012/2024-07-10/2024-07-10/text/original/epub/OEBPS/document_1/document_1.html#_Toc172118921> ;
    dcat:landingPage "https://www.legislation.gov.au/C2020A00012/2024-07-10/2024-07-10/text/original/epub/OEBPS/document_1/document_1.html#_Toc172118921"^^xsd:anyURI ;
    dcat:theme legcons:Subdivision .

C2020A00012:250 a legcons:Division,
        owl:Class,
        dcat:Resource ;
    rdfs:label "Division - D250 Division 1 Revocation requested by holder"@en-AU ;
    dct:hasPart C2020A00012:251 ;
    dct:isPartOf C2020A00012:249 ;
    dct:isReferencedBy C2020A00012: ;
    rdfs:comment "Division 1 Revocation requested by holder - Abrievated Graph Key: D250"@en-AU ;
    skos:broader C2020A00012:251 ;
    skos:definition "Division 1 Revocation requested by holder"@en-AU ;
    skos:narrower C2020A00012:249 ;
    skos:prefLabel "Division D250"@en-AU ;
    dcat:accessURL <https://www.legislation.gov.au/C2020A00012/2024-07-10/2024-07-10/text/original/epub/OEBPS/document_1/document_1.html#_Toc172118942> ;
    dcat:landingPage "https://www.legislation.gov.au/C2020A00012/2024-07-10/2024-07-10/text/original/epub/OEBPS/document_1/document_1.html#_Toc172118942"^^xsd:anyURI ;
    dcat:theme legcons:Division .

C2020A00012:266 a legcons:Part,
        owl:Class,
        dcat:Resource ;
    rdfs:label "Part - P266 Part 1 Introduction"@en-AU ;
    dct:hasPart C2020A00012:267 ;
    dct:isPartOf C2020A00012:265 ;
    dct:isReferencedBy C2020A00012: ;
    rdfs:comment "Part 1 Introduction - Abrievated Graph Key: P266"@en-AU ;
    skos:broader C2020A00012:267 ;
    skos:definition "Part 1 Introduction"@en-AU ;
    skos:narrower C2020A00012:265 ;
    skos:prefLabel "Part P266"@en-AU ;
    dcat:accessURL <https://www.legislation.gov.au/C2020A00012/2024-07-10/2024-07-10/text/original/epub/OEBPS/document_1/document_1.html#_Toc172118958> ;
    dcat:landingPage "https://www.legislation.gov.au/C2020A00012/2024-07-10/2024-07-10/text/original/epub/OEBPS/document_1/document_1.html#_Toc172118958"^^xsd:anyURI ;
    dcat:theme legcons:Part .

C2020A00012:29 a legcons:Division,
        owl:Class,
        dcat:Resource ;
    rdfs:label "Division - D29 Division 1 Introduction"@en-AU ;
    dct:hasPart C2020A00012:30 ;
    dct:isPartOf C2020A00012:28 ;
    dct:isReferencedBy C2020A00012: ;
    rdfs:comment "Division 1 Introduction - Abrievated Graph Key: D29"@en-AU ;
    skos:broader C2020A00012:30 ;
    skos:definition "Division 1 Introduction"@en-AU ;
    skos:narrower C2020A00012:28 ;
    skos:prefLabel "Division D29"@en-AU ;
    dcat:accessURL <https://www.legislation.gov.au/C2020A00012/2024-07-10/2024-07-10/text/original/epub/OEBPS/document_1/document_1.html#_Toc172118721> ;
    dcat:landingPage "https://www.legislation.gov.au/C2020A00012/2024-07-10/2024-07-10/text/original/epub/OEBPS/document_1/document_1.html#_Toc172118721"^^xsd:anyURI ;
    dcat:theme legcons:Division .

C2020A00012:296 a legcons:Division,
        owl:Class,
        dcat:Resource ;
    rdfs:label "Division - D296 Division 3 Other provisions"@en-AU ;
    dct:hasPart C2020A00012:297 ;
    dct:isPartOf C2020A00012:286 ;
    dct:isReferencedBy C2020A00012: ;
    rdfs:comment "Division 3 Other provisions - Abrievated Graph Key: D296"@en-AU ;
    skos:broader C2020A00012:297 ;
    skos:definition "Division 3 Other provisions"@en-AU ;
    skos:narrower C2020A00012:286 ;
    skos:prefLabel "Division D296"@en-AU ;
    dcat:accessURL <https://www.legislation.gov.au/C2020A00012/2024-07-10/2024-07-10/text/original/epub/OEBPS/document_1/document_1.html#_Toc172118988> ;
    dcat:landingPage "https://www.legislation.gov.au/C2020A00012/2024-07-10/2024-07-10/text/original/epub/OEBPS/document_1/document_1.html#_Toc172118988"^^xsd:anyURI ;
    dcat:theme legcons:Division .

C2020A00012:299 a legcons:Division,
        owl:Class,
        dcat:Resource ;
    rdfs:label "Division - D299 Division 1 Revocation requested by holder"@en-AU ;
    dct:hasPart C2020A00012:300 ;
    dct:isPartOf C2020A00012:298 ;
    dct:isReferencedBy C2020A00012: ;
    rdfs:comment "Division 1 Revocation requested by holder - Abrievated Graph Key: D299"@en-AU ;
    skos:broader C2020A00012:300 ;
    skos:definition "Division 1 Revocation requested by holder"@en-AU ;
    skos:narrower C2020A00012:298 ;
    skos:prefLabel "Division D299"@en-AU ;
    dcat:accessURL <https://www.legislation.gov.au/C2020A00012/2024-07-10/2024-07-10/text/original/epub/OEBPS/document_1/document_1.html#_Toc172118991> ;
    dcat:landingPage "https://www.legislation.gov.au/C2020A00012/2024-07-10/2024-07-10/text/original/epub/OEBPS/document_1/document_1.html#_Toc172118991"^^xsd:anyURI ;
    dcat:theme legcons:Division .

C2020A00012:317 a legcons:Part,
        owl:Class,
        dcat:Resource ;
    rdfs:label "Part - P317 Part 1 Introduction"@en-AU ;
    dct:hasPart C2020A00012:318 ;
    dct:isPartOf C2020A00012:316 ;
    dct:isReferencedBy C2020A00012: ;
    rdfs:comment "Part 1 Introduction - Abrievated Graph Key: P317"@en-AU ;
    skos:broader C2020A00012:318 ;
    skos:definition "Part 1 Introduction"@en-AU ;
    skos:narrower C2020A00012:316 ;
    skos:prefLabel "Part P317"@en-AU ;
    dcat:accessURL <https://www.legislation.gov.au/C2020A00012/2024-07-10/2024-07-10/text/original/epub/OEBPS/document_1/document_1.html#_Toc172119009> ;
    dcat:landingPage "https://www.legislation.gov.au/C2020A00012/2024-07-10/2024-07-10/text/original/epub/OEBPS/document_1/document_1.html#_Toc172119009"^^xsd:anyURI ;
    dcat:theme legcons:Part .

C2020A00012:343 a legcons:Division,
        owl:Class,
        dcat:Resource ;
    rdfs:label "Division - D343 Division 1 Introduction"@en-AU ;
    dct:hasPart C2020A00012:344 ;
    dct:isPartOf C2020A00012:342 ;
    dct:isReferencedBy C2020A00012: ;
    rdfs:comment "Division 1 Introduction - Abrievated Graph Key: D343"@en-AU ;
    skos:broader C2020A00012:344 ;
    skos:definition "Division 1 Introduction"@en-AU ;
    skos:narrower C2020A00012:342 ;
    skos:prefLabel "Division D343"@en-AU ;
    dcat:accessURL <https://www.legislation.gov.au/C2020A00012/2024-07-10/2024-07-10/text/original/epub/OEBPS/document_1/document_1.html#_Toc172119035> ;
    dcat:landingPage "https://www.legislation.gov.au/C2020A00012/2024-07-10/2024-07-10/text/original/epub/OEBPS/document_1/document_1.html#_Toc172119035"^^xsd:anyURI ;
    dcat:theme legcons:Division .

C2020A00012:349 a legcons:Division,
        owl:Class,
        dcat:Resource ;
    rdfs:label "Division - D349 Division 1 Introduction"@en-AU ;
    dct:hasPart C2020A00012:350 ;
    dct:isPartOf C2020A00012:348 ;
    dct:isReferencedBy C2020A00012: ;
    rdfs:comment "Division 1 Introduction - Abrievated Graph Key: D349"@en-AU ;
    skos:broader C2020A00012:350 ;
    skos:definition "Division 1 Introduction"@en-AU ;
    skos:narrower C2020A00012:348 ;
    skos:prefLabel "Division D349"@en-AU ;
    dcat:accessURL <https://www.legislation.gov.au/C2020A00012/2024-07-10/2024-07-10/text/original/epub/OEBPS/document_1/document_1.html#_Toc172119041> ;
    dcat:landingPage "https://www.legislation.gov.au/C2020A00012/2024-07-10/2024-07-10/text/original/epub/OEBPS/document_1/document_1.html#_Toc172119041"^^xsd:anyURI ;
    dcat:theme legcons:Division .

C2020A00012:362 a legcons:Division,
        owl:Class,
        dcat:Resource ;
    rdfs:label "Division - D362 Division 1 Introduction"@en-AU ;
    dct:hasPart C2020A00012:363 ;
    dct:isPartOf C2020A00012:361 ;
    dct:isReferencedBy C2020A00012: ;
    rdfs:comment "Division 1 Introduction - Abrievated Graph Key: D362"@en-AU ;
    skos:broader C2020A00012:363 ;
    skos:definition "Division 1 Introduction"@en-AU ;
    skos:narrower C2020A00012:361 ;
    skos:prefLabel "Division D362"@en-AU ;
    dcat:accessURL <https://www.legislation.gov.au/C2020A00012/2024-07-10/2024-07-10/text/original/epub/OEBPS/document_1/document_1.html#_Toc172119054> ;
    dcat:landingPage "https://www.legislation.gov.au/C2020A00012/2024-07-10/2024-07-10/text/original/epub/OEBPS/document_1/document_1.html#_Toc172119054"^^xsd:anyURI ;
    dcat:theme legcons:Division .

C2020A00012:375 a legcons:Division,
        owl:Class,
        dcat:Resource ;
    rdfs:label "Division - D375 Division 1 Introduction"@en-AU ;
    dct:hasPart C2020A00012:376 ;
    dct:isPartOf C2020A00012:374 ;
    dct:isReferencedBy C2020A00012: ;
    rdfs:comment "Division 1 Introduction - Abrievated Graph Key: D375"@en-AU ;
    skos:broader C2020A00012:376 ;
    skos:definition "Division 1 Introduction"@en-AU ;
    skos:narrower C2020A00012:374 ;
    skos:prefLabel "Division D375"@en-AU ;
    dcat:accessURL <https://www.legislation.gov.au/C2020A00012/2024-07-10/2024-07-10/text/original/epub/OEBPS/document_1/document_1.html#_Toc172119067> ;
    dcat:landingPage "https://www.legislation.gov.au/C2020A00012/2024-07-10/2024-07-10/text/original/epub/OEBPS/document_1/document_1.html#_Toc172119067"^^xsd:anyURI ;
    dcat:theme legcons:Division .

C2020A00012:377 a legcons:Division,
        owl:Class,
        dcat:Resource ;
    rdfs:label "Division - D377 Division 2 Tariff rate quota systems"@en-AU ;
    dct:hasPart C2020A00012:378 ;
    dct:isPartOf C2020A00012:374 ;
    dct:isReferencedBy C2020A00012: ;
    rdfs:comment "Division 2 Tariff rate quota systems - Abrievated Graph Key: D377"@en-AU ;
    skos:broader C2020A00012:378 ;
    skos:definition "Division 2 Tariff rate quota systems"@en-AU ;
    skos:narrower C2020A00012:374 ;
    skos:prefLabel "Division D377"@en-AU ;
    dcat:accessURL <https://www.legislation.gov.au/C2020A00012/2024-07-10/2024-07-10/text/original/epub/OEBPS/document_1/document_1.html#_Toc172119069> ;
    dcat:landingPage "https://www.legislation.gov.au/C2020A00012/2024-07-10/2024-07-10/text/original/epub/OEBPS/document_1/document_1.html#_Toc172119069"^^xsd:anyURI ;
    dcat:theme legcons:Division .

C2020A00012:381 a legcons:Division,
        owl:Class,
        dcat:Resource ;
    rdfs:label "Division - D381 Division 1 Introduction"@en-AU ;
    dct:hasPart C2020A00012:382 ;
    dct:isPartOf C2020A00012:380 ;
    dct:isReferencedBy C2020A00012: ;
    rdfs:comment "Division 1 Introduction - Abrievated Graph Key: D381"@en-AU ;
    skos:broader C2020A00012:382 ;
    skos:definition "Division 1 Introduction"@en-AU ;
    skos:narrower C2020A00012:380 ;
    skos:prefLabel "Division D381"@en-AU ;
    dcat:accessURL <https://www.legislation.gov.au/C2020A00012/2024-07-10/2024-07-10/text/original/epub/OEBPS/document_1/document_1.html#_Toc172119073> ;
    dcat:landingPage "https://www.legislation.gov.au/C2020A00012/2024-07-10/2024-07-10/text/original/epub/OEBPS/document_1/document_1.html#_Toc172119073"^^xsd:anyURI ;
    dcat:theme legcons:Division .

C2020A00012:396 a legcons:Division,
        owl:Class,
        dcat:Resource ;
    rdfs:label "Division - D396 Division 1 Introduction"@en-AU ;
    dct:hasPart C2020A00012:397 ;
    dct:isPartOf C2020A00012:395 ;
    dct:isReferencedBy C2020A00012: ;
    rdfs:comment "Division 1 Introduction - Abrievated Graph Key: D396"@en-AU ;
    skos:broader C2020A00012:397 ;
    skos:definition "Division 1 Introduction"@en-AU ;
    skos:narrower C2020A00012:395 ;
    skos:prefLabel "Division D396"@en-AU ;
    dcat:accessURL <https://www.legislation.gov.au/C2020A00012/2024-07-10/2024-07-10/text/original/epub/OEBPS/document_1/document_1.html#_Toc172119088> ;
    dcat:landingPage "https://www.legislation.gov.au/C2020A00012/2024-07-10/2024-07-10/text/original/epub/OEBPS/document_1/document_1.html#_Toc172119088"^^xsd:anyURI ;
    dcat:theme legcons:Division .

C2020A00012:408 a legcons:Division,
        owl:Class,
        dcat:Resource ;
    rdfs:label "Division - D408 Division 1 Introduction"@en-AU ;
    dct:hasPart C2020A00012:409 ;
    dct:isPartOf C2020A00012:407 ;
    dct:isReferencedBy C2020A00012: ;
    rdfs:comment "Division 1 Introduction - Abrievated Graph Key: D408"@en-AU ;
    skos:broader C2020A00012:409 ;
    skos:definition "Division 1 Introduction"@en-AU ;
    skos:narrower C2020A00012:407 ;
    skos:prefLabel "Division D408"@en-AU ;
    dcat:accessURL <https://www.legislation.gov.au/C2020A00012/2024-07-10/2024-07-10/text/original/epub/OEBPS/document_1/document_1.html#_Toc172119100> ;
    dcat:landingPage "https://www.legislation.gov.au/C2020A00012/2024-07-10/2024-07-10/text/original/epub/OEBPS/document_1/document_1.html#_Toc172119100"^^xsd:anyURI ;
    dcat:theme legcons:Division .

C2020A00012:417 a legcons:Division,
        owl:Class,
        dcat:Resource ;
    rdfs:label "Division - D417 Division 1 Introduction"@en-AU ;
    dct:hasPart C2020A00012:418 ;
    dct:isPartOf C2020A00012:416 ;
    dct:isReferencedBy C2020A00012: ;
    rdfs:comment "Division 1 Introduction - Abrievated Graph Key: D417"@en-AU ;
    skos:broader C2020A00012:418 ;
    skos:definition "Division 1 Introduction"@en-AU ;
    skos:narrower C2020A00012:416 ;
    skos:prefLabel "Division D417"@en-AU ;
    dcat:accessURL <https://www.legislation.gov.au/C2020A00012/2024-07-10/2024-07-10/text/original/epub/OEBPS/document_1/document_1.html#_Toc172119109> ;
    dcat:landingPage "https://www.legislation.gov.au/C2020A00012/2024-07-10/2024-07-10/text/original/epub/OEBPS/document_1/document_1.html#_Toc172119109"^^xsd:anyURI ;
    dcat:theme legcons:Division .

C2020A00012:435 a legcons:Subdivision,
        owl:Class,
        dcat:Resource ;
    rdfs:label "Subdivision - S435 Subdivision COther provisions"@en-AU ;
    dct:hasPart C2020A00012:436 ;
    dct:isPartOf C2020A00012:424 ;
    dct:isReferencedBy C2020A00012: ;
    rdfs:comment "Subdivision COther provisions - Abrievated Graph Key: S435"@en-AU ;
    skos:broader C2020A00012:436 ;
    skos:definition "Subdivision COther provisions"@en-AU ;
    skos:narrower C2020A00012:424 ;
    skos:prefLabel "Subdivision S435"@en-AU ;
    dcat:accessURL <https://www.legislation.gov.au/C2020A00012/2024-07-10/2024-07-10/text/original/epub/OEBPS/document_1/document_1.html#_Toc172119127> ;
    dcat:landingPage "https://www.legislation.gov.au/C2020A00012/2024-07-10/2024-07-10/text/original/epub/OEBPS/document_1/document_1.html#_Toc172119127"^^xsd:anyURI ;
    dcat:theme legcons:Subdivision .

C2020A00012:450 a legcons:Division,
        owl:Class,
        dcat:Resource ;
    rdfs:label "Division - D450 Division 1 Introduction"@en-AU ;
    dct:hasPart C2020A00012:451 ;
    dct:isPartOf C2020A00012:449 ;
    dct:isReferencedBy C2020A00012: ;
    rdfs:comment "Division 1 Introduction - Abrievated Graph Key: D450"@en-AU ;
    skos:broader C2020A00012:451 ;
    skos:definition "Division 1 Introduction"@en-AU ;
    skos:narrower C2020A00012:449 ;
    skos:prefLabel "Division D450"@en-AU ;
    dcat:accessURL <https://www.legislation.gov.au/C2020A00012/2024-07-10/2024-07-10/text/original/epub/OEBPS/document_1/document_1.html#_Toc172119142> ;
    dcat:landingPage "https://www.legislation.gov.au/C2020A00012/2024-07-10/2024-07-10/text/original/epub/OEBPS/document_1/document_1.html#_Toc172119142"^^xsd:anyURI ;
    dcat:theme legcons:Division .

C2020A00012:465 a legcons:Division,
        owl:Class,
        dcat:Resource ;
    rdfs:label "Division - D465 Division 4 Extended geographical operation of offences"@en-AU ;
    dct:hasPart C2020A00012:466 ;
    dct:isPartOf C2020A00012:449 ;
    dct:isReferencedBy C2020A00012: ;
    rdfs:comment "Division 4 Extended geographical operation of offences - Abrievated Graph Key: D465"@en-AU ;
    skos:broader C2020A00012:466 ;
    skos:definition "Division 4 Extended geographical operation of offences"@en-AU ;
    skos:narrower C2020A00012:449 ;
    skos:prefLabel "Division D465"@en-AU ;
    dcat:accessURL <https://www.legislation.gov.au/C2020A00012/2024-07-10/2024-07-10/text/original/epub/OEBPS/document_1/document_1.html#_Toc172119157> ;
    dcat:landingPage "https://www.legislation.gov.au/C2020A00012/2024-07-10/2024-07-10/text/original/epub/OEBPS/document_1/document_1.html#_Toc172119157"^^xsd:anyURI ;
    dcat:theme legcons:Division .

C2020A00012:472 a legcons:Division,
        owl:Class,
        dcat:Resource ;
    rdfs:label "Division - D472 Division 1 Introduction"@en-AU ;
    dct:hasPart C2020A00012:473 ;
    dct:isPartOf C2020A00012:471 ;
    dct:isReferencedBy C2020A00012: ;
    rdfs:comment "Division 1 Introduction - Abrievated Graph Key: D472"@en-AU ;
    skos:broader C2020A00012:473 ;
    skos:definition "Division 1 Introduction"@en-AU ;
    skos:narrower C2020A00012:471 ;
    skos:prefLabel "Division D472"@en-AU ;
    dcat:accessURL <https://www.legislation.gov.au/C2020A00012/2024-07-10/2024-07-10/text/original/epub/OEBPS/document_1/document_1.html#_Toc172119164> ;
    dcat:landingPage "https://www.legislation.gov.au/C2020A00012/2024-07-10/2024-07-10/text/original/epub/OEBPS/document_1/document_1.html#_Toc172119164"^^xsd:anyURI ;
    dcat:theme legcons:Division .

C2020A00012:478 a legcons:Division,
        owl:Class,
        dcat:Resource ;
    rdfs:label "Division - D478 Division 1 Introduction"@en-AU ;
    dct:hasPart C2020A00012:479 ;
    dct:isPartOf C2020A00012:477 ;
    dct:isReferencedBy C2020A00012: ;
    rdfs:comment "Division 1 Introduction - Abrievated Graph Key: D478"@en-AU ;
    skos:broader C2020A00012:479 ;
    skos:definition "Division 1 Introduction"@en-AU ;
    skos:narrower C2020A00012:477 ;
    skos:prefLabel "Division D478"@en-AU ;
    dcat:accessURL <https://www.legislation.gov.au/C2020A00012/2024-07-10/2024-07-10/text/original/epub/OEBPS/document_1/document_1.html#_Toc172119170> ;
    dcat:landingPage "https://www.legislation.gov.au/C2020A00012/2024-07-10/2024-07-10/text/original/epub/OEBPS/document_1/document_1.html#_Toc172119170"^^xsd:anyURI ;
    dcat:theme legcons:Division .

C2020A00012:490 a legcons:Division,
        owl:Class,
        dcat:Resource ;
    rdfs:label "Division - D490 Division 3 Adjacent premises warrants"@en-AU ;
    dct:hasPart C2020A00012:491 ;
    dct:isPartOf C2020A00012:483 ;
    dct:isReferencedBy C2020A00012: ;
    rdfs:comment "Division 3 Adjacent premises warrants - Abrievated Graph Key: D490"@en-AU ;
    skos:broader C2020A00012:491 ;
    skos:definition "Division 3 Adjacent premises warrants"@en-AU ;
    skos:narrower C2020A00012:483 ;
    skos:prefLabel "Division D490"@en-AU ;
    dcat:accessURL <https://www.legislation.gov.au/C2020A00012/2024-07-10/2024-07-10/text/original/epub/OEBPS/document_1/document_1.html#_Toc172119182> ;
    dcat:landingPage "https://www.legislation.gov.au/C2020A00012/2024-07-10/2024-07-10/text/original/epub/OEBPS/document_1/document_1.html#_Toc172119182"^^xsd:anyURI ;
    dcat:theme legcons:Division .

C2020A00012:501 a legcons:Division,
        owl:Class,
        dcat:Resource ;
    rdfs:label "Division - D501 Division 6 Powers of issuing officers"@en-AU ;
    dct:hasPart C2020A00012:502 ;
    dct:isPartOf C2020A00012:483 ;
    dct:isReferencedBy C2020A00012: ;
    rdfs:comment "Division 6 Powers of issuing officers - Abrievated Graph Key: D501"@en-AU ;
    skos:broader C2020A00012:502 ;
    skos:definition "Division 6 Powers of issuing officers"@en-AU ;
    skos:narrower C2020A00012:483 ;
    skos:prefLabel "Division D501"@en-AU ;
    dcat:accessURL <https://www.legislation.gov.au/C2020A00012/2024-07-10/2024-07-10/text/original/epub/OEBPS/document_1/document_1.html#_Toc172119193> ;
    dcat:landingPage "https://www.legislation.gov.au/C2020A00012/2024-07-10/2024-07-10/text/original/epub/OEBPS/document_1/document_1.html#_Toc172119193"^^xsd:anyURI ;
    dcat:theme legcons:Division .

C2020A00012:517 a legcons:Division,
        owl:Class,
        dcat:Resource ;
    rdfs:label "Division - D517 Division 1 Introduction"@en-AU ;
    dct:hasPart C2020A00012:518 ;
    dct:isPartOf C2020A00012:516 ;
    dct:isReferencedBy C2020A00012: ;
    rdfs:comment "Division 1 Introduction - Abrievated Graph Key: D517"@en-AU ;
    skos:broader C2020A00012:518 ;
    skos:definition "Division 1 Introduction"@en-AU ;
    skos:narrower C2020A00012:516 ;
    skos:prefLabel "Division D517"@en-AU ;
    dcat:accessURL <https://www.legislation.gov.au/C2020A00012/2024-07-10/2024-07-10/text/original/epub/OEBPS/document_1/document_1.html#_Toc172119209> ;
    dcat:landingPage "https://www.legislation.gov.au/C2020A00012/2024-07-10/2024-07-10/text/original/epub/OEBPS/document_1/document_1.html#_Toc172119209"^^xsd:anyURI ;
    dcat:theme legcons:Division .

C2020A00012:523 a legcons:Division,
        owl:Class,
        dcat:Resource ;
    rdfs:label "Division - D523 Division 1 Introduction"@en-AU ;
    dct:hasPart C2020A00012:524 ;
    dct:isPartOf C2020A00012:522 ;
    dct:isReferencedBy C2020A00012: ;
    rdfs:comment "Division 1 Introduction - Abrievated Graph Key: D523"@en-AU ;
    skos:broader C2020A00012:524 ;
    skos:definition "Division 1 Introduction"@en-AU ;
    skos:narrower C2020A00012:522 ;
    skos:prefLabel "Division D523"@en-AU ;
    dcat:accessURL <https://www.legislation.gov.au/C2020A00012/2024-07-10/2024-07-10/text/original/epub/OEBPS/document_1/document_1.html#_Toc172119215> ;
    dcat:landingPage "https://www.legislation.gov.au/C2020A00012/2024-07-10/2024-07-10/text/original/epub/OEBPS/document_1/document_1.html#_Toc172119215"^^xsd:anyURI ;
    dcat:theme legcons:Division .

C2020A00012:525 a legcons:Division,
        owl:Class,
        dcat:Resource ;
    rdfs:label "Division - D525 Division 2 Civil penalties under Part 4 of the Regulatory Powers Act"@en-AU ;
    dct:hasPart C2020A00012:526 ;
    dct:isPartOf C2020A00012:522 ;
    dct:isReferencedBy C2020A00012: ;
    rdfs:comment "Division 2 Civil penalties under Part 4 of the Regulatory Powers Act - Abrievated Graph Key: D525"@en-AU ;
    skos:broader C2020A00012:526 ;
    skos:definition "Division 2 Civil penalties under Part 4 of the Regulatory Powers Act"@en-AU ;
    skos:narrower C2020A00012:522 ;
    skos:prefLabel "Division D525"@en-AU ;
    dcat:accessURL <https://www.legislation.gov.au/C2020A00012/2024-07-10/2024-07-10/text/original/epub/OEBPS/document_1/document_1.html#_Toc172119217> ;
    dcat:landingPage "https://www.legislation.gov.au/C2020A00012/2024-07-10/2024-07-10/text/original/epub/OEBPS/document_1/document_1.html#_Toc172119217"^^xsd:anyURI ;
    dcat:theme legcons:Division .

C2020A00012:528 a legcons:Division,
        owl:Class,
        dcat:Resource ;
    rdfs:label "Division - D528 Division 1 Introduction"@en-AU ;
    dct:hasPart C2020A00012:529 ;
    dct:isPartOf C2020A00012:527 ;
    dct:isReferencedBy C2020A00012: ;
    rdfs:comment "Division 1 Introduction - Abrievated Graph Key: D528"@en-AU ;
    skos:broader C2020A00012:529 ;
    skos:definition "Division 1 Introduction"@en-AU ;
    skos:narrower C2020A00012:527 ;
    skos:prefLabel "Division D528"@en-AU ;
    dcat:accessURL <https://www.legislation.gov.au/C2020A00012/2024-07-10/2024-07-10/text/original/epub/OEBPS/document_1/document_1.html#_Toc172119220> ;
    dcat:landingPage "https://www.legislation.gov.au/C2020A00012/2024-07-10/2024-07-10/text/original/epub/OEBPS/document_1/document_1.html#_Toc172119220"^^xsd:anyURI ;
    dcat:theme legcons:Division .

C2020A00012:534 a legcons:Division,
        owl:Class,
        dcat:Resource ;
    rdfs:label "Division - D534 Division 1 Introduction"@en-AU ;
    dct:hasPart C2020A00012:535 ;
    dct:isPartOf C2020A00012:533 ;
    dct:isReferencedBy C2020A00012: ;
    rdfs:comment "Division 1 Introduction - Abrievated Graph Key: D534"@en-AU ;
    skos:broader C2020A00012:535 ;
    skos:definition "Division 1 Introduction"@en-AU ;
    skos:narrower C2020A00012:533 ;
    skos:prefLabel "Division D534"@en-AU ;
    dcat:accessURL <https://www.legislation.gov.au/C2020A00012/2024-07-10/2024-07-10/text/original/epub/OEBPS/document_1/document_1.html#_Toc172119226> ;
    dcat:landingPage "https://www.legislation.gov.au/C2020A00012/2024-07-10/2024-07-10/text/original/epub/OEBPS/document_1/document_1.html#_Toc172119226"^^xsd:anyURI ;
    dcat:theme legcons:Division .

C2020A00012:536 a legcons:Division,
        owl:Class,
        dcat:Resource ;
    rdfs:label "Division - D536 Division 2 Accepting and enforcing undertakings under Part 6 of the Regulatory Powers Act"@en-AU ;
    dct:hasPart C2020A00012:537 ;
    dct:isPartOf C2020A00012:533 ;
    dct:isReferencedBy C2020A00012: ;
    rdfs:comment "Division 2 Accepting and enforcing undertakings under Part 6 of the Regulatory Powers Act - Abrievated Graph Key: D536"@en-AU ;
    skos:broader C2020A00012:537 ;
    skos:definition "Division 2 Accepting and enforcing undertakings under Part 6 of the Regulatory Powers Act"@en-AU ;
    skos:narrower C2020A00012:533 ;
    skos:prefLabel "Division D536"@en-AU ;
    dcat:accessURL <https://www.legislation.gov.au/C2020A00012/2024-07-10/2024-07-10/text/original/epub/OEBPS/document_1/document_1.html#_Toc172119228> ;
    dcat:landingPage "https://www.legislation.gov.au/C2020A00012/2024-07-10/2024-07-10/text/original/epub/OEBPS/document_1/document_1.html#_Toc172119228"^^xsd:anyURI ;
    dcat:theme legcons:Division .

C2020A00012:539 a legcons:Division,
        owl:Class,
        dcat:Resource ;
    rdfs:label "Division - D539 Division 1 Introduction"@en-AU ;
    dct:hasPart C2020A00012:540 ;
    dct:isPartOf C2020A00012:538 ;
    dct:isReferencedBy C2020A00012: ;
    rdfs:comment "Division 1 Introduction - Abrievated Graph Key: D539"@en-AU ;
    skos:broader C2020A00012:540 ;
    skos:definition "Division 1 Introduction"@en-AU ;
    skos:narrower C2020A00012:538 ;
    skos:prefLabel "Division D539"@en-AU ;
    dcat:accessURL <https://www.legislation.gov.au/C2020A00012/2024-07-10/2024-07-10/text/original/epub/OEBPS/document_1/document_1.html#_Toc172119231> ;
    dcat:landingPage "https://www.legislation.gov.au/C2020A00012/2024-07-10/2024-07-10/text/original/epub/OEBPS/document_1/document_1.html#_Toc172119231"^^xsd:anyURI ;
    dcat:theme legcons:Division .

C2020A00012:541 a legcons:Division,
        owl:Class,
        dcat:Resource ;
    rdfs:label "Division - D541 Division 2 Injunctions under Part 7 of the Regulatory Powers Act"@en-AU ;
    dct:hasPart C2020A00012:542 ;
    dct:isPartOf C2020A00012:538 ;
    dct:isReferencedBy C2020A00012: ;
    rdfs:comment "Division 2 Injunctions under Part 7 of the Regulatory Powers Act - Abrievated Graph Key: D541"@en-AU ;
    skos:broader C2020A00012:542 ;
    skos:definition "Division 2 Injunctions under Part 7 of the Regulatory Powers Act"@en-AU ;
    skos:narrower C2020A00012:538 ;
    skos:prefLabel "Division D541"@en-AU ;
    dcat:accessURL <https://www.legislation.gov.au/C2020A00012/2024-07-10/2024-07-10/text/original/epub/OEBPS/document_1/document_1.html#_Toc172119233> ;
    dcat:landingPage "https://www.legislation.gov.au/C2020A00012/2024-07-10/2024-07-10/text/original/epub/OEBPS/document_1/document_1.html#_Toc172119233"^^xsd:anyURI ;
    dcat:theme legcons:Division .

C2020A00012:551 a legcons:Division,
        owl:Class,
        dcat:Resource ;
    rdfs:label "Division - D551 Division 1 Introduction"@en-AU ;
    dct:hasPart C2020A00012:552 ;
    dct:isPartOf C2020A00012:550 ;
    dct:isReferencedBy C2020A00012: ;
    rdfs:comment "Division 1 Introduction - Abrievated Graph Key: D551"@en-AU ;
    skos:broader C2020A00012:552 ;
    skos:definition "Division 1 Introduction"@en-AU ;
    skos:narrower C2020A00012:550 ;
    skos:prefLabel "Division D551"@en-AU ;
    dcat:accessURL <https://www.legislation.gov.au/C2020A00012/2024-07-10/2024-07-10/text/original/epub/OEBPS/document_1/document_1.html#_Toc172119243> ;
    dcat:landingPage "https://www.legislation.gov.au/C2020A00012/2024-07-10/2024-07-10/text/original/epub/OEBPS/document_1/document_1.html#_Toc172119243"^^xsd:anyURI ;
    dcat:theme legcons:Division .

C2020A00012:553 a legcons:Division,
        owl:Class,
        dcat:Resource ;
    rdfs:label "Division - D553 Division 2 Persons assisting authorised officers"@en-AU ;
    dct:hasPart C2020A00012:554 ;
    dct:isPartOf C2020A00012:550 ;
    dct:isReferencedBy C2020A00012: ;
    rdfs:comment "Division 2 Persons assisting authorised officers - Abrievated Graph Key: D553"@en-AU ;
    skos:broader C2020A00012:554 ;
    skos:definition "Division 2 Persons assisting authorised officers"@en-AU ;
    skos:narrower C2020A00012:550 ;
    skos:prefLabel "Division D553"@en-AU ;
    dcat:accessURL <https://www.legislation.gov.au/C2020A00012/2024-07-10/2024-07-10/text/original/epub/OEBPS/document_1/document_1.html#_Toc172119245> ;
    dcat:landingPage "https://www.legislation.gov.au/C2020A00012/2024-07-10/2024-07-10/text/original/epub/OEBPS/document_1/document_1.html#_Toc172119245"^^xsd:anyURI ;
    dcat:theme legcons:Division .

C2020A00012:568 a legcons:Division,
        owl:Class,
        dcat:Resource ;
    rdfs:label "Division - D568 Division 1 Introduction"@en-AU ;
    dct:hasPart C2020A00012:569 ;
    dct:isPartOf C2020A00012:567 ;
    dct:isReferencedBy C2020A00012: ;
    rdfs:comment "Division 1 Introduction - Abrievated Graph Key: D568"@en-AU ;
    skos:broader C2020A00012:569 ;
    skos:definition "Division 1 Introduction"@en-AU ;
    skos:narrower C2020A00012:567 ;
    skos:prefLabel "Division D568"@en-AU ;
    dcat:accessURL <https://www.legislation.gov.au/C2020A00012/2024-07-10/2024-07-10/text/original/epub/OEBPS/document_1/document_1.html#_Toc172119260> ;
    dcat:landingPage "https://www.legislation.gov.au/C2020A00012/2024-07-10/2024-07-10/text/original/epub/OEBPS/document_1/document_1.html#_Toc172119260"^^xsd:anyURI ;
    dcat:theme legcons:Division .

C2020A00012:576 a legcons:Division,
        owl:Class,
        dcat:Resource ;
    rdfs:label "Division - D576 Division 1 Introduction"@en-AU ;
    dct:hasPart C2020A00012:577 ;
    dct:isPartOf C2020A00012:575 ;
    dct:isReferencedBy C2020A00012: ;
    rdfs:comment "Division 1 Introduction - Abrievated Graph Key: D576"@en-AU ;
    skos:broader C2020A00012:577 ;
    skos:definition "Division 1 Introduction"@en-AU ;
    skos:narrower C2020A00012:575 ;
    skos:prefLabel "Division D576"@en-AU ;
    dcat:accessURL <https://www.legislation.gov.au/C2020A00012/2024-07-10/2024-07-10/text/original/epub/OEBPS/document_1/document_1.html#_Toc172119268> ;
    dcat:landingPage "https://www.legislation.gov.au/C2020A00012/2024-07-10/2024-07-10/text/original/epub/OEBPS/document_1/document_1.html#_Toc172119268"^^xsd:anyURI ;
    dcat:theme legcons:Division .

C2020A00012:582 a legcons:Division,
        owl:Class,
        dcat:Resource ;
    rdfs:label "Division - D582 Division 1 Introduction"@en-AU ;
    dct:hasPart C2020A00012:583 ;
    dct:isPartOf C2020A00012:581 ;
    dct:isReferencedBy C2020A00012: ;
    rdfs:comment "Division 1 Introduction - Abrievated Graph Key: D582"@en-AU ;
    skos:broader C2020A00012:583 ;
    skos:definition "Division 1 Introduction"@en-AU ;
    skos:narrower C2020A00012:581 ;
    skos:prefLabel "Division D582"@en-AU ;
    dcat:accessURL <https://www.legislation.gov.au/C2020A00012/2024-07-10/2024-07-10/text/original/epub/OEBPS/document_1/document_1.html#_Toc172119274> ;
    dcat:landingPage "https://www.legislation.gov.au/C2020A00012/2024-07-10/2024-07-10/text/original/epub/OEBPS/document_1/document_1.html#_Toc172119274"^^xsd:anyURI ;
    dcat:theme legcons:Division .

C2020A00012:592 a legcons:Division,
        owl:Class,
        dcat:Resource ;
    rdfs:label "Division - D592 Division 1 Introduction"@en-AU ;
    dct:hasPart C2020A00012:593 ;
    dct:isPartOf C2020A00012:591 ;
    dct:isReferencedBy C2020A00012: ;
    rdfs:comment "Division 1 Introduction - Abrievated Graph Key: D592"@en-AU ;
    skos:broader C2020A00012:593 ;
    skos:definition "Division 1 Introduction"@en-AU ;
    skos:narrower C2020A00012:591 ;
    skos:prefLabel "Division D592"@en-AU ;
    dcat:accessURL <https://www.legislation.gov.au/C2020A00012/2024-07-10/2024-07-10/text/original/epub/OEBPS/document_1/document_1.html#_Toc172119284> ;
    dcat:landingPage "https://www.legislation.gov.au/C2020A00012/2024-07-10/2024-07-10/text/original/epub/OEBPS/document_1/document_1.html#_Toc172119284"^^xsd:anyURI ;
    dcat:theme legcons:Division .

C2020A00012:614 a legcons:Division,
        owl:Class,
        dcat:Resource ;
    rdfs:label "Division - D614 Division 1 Introduction"@en-AU ;
    dct:hasPart C2020A00012:615 ;
    dct:isPartOf C2020A00012:613 ;
    dct:isReferencedBy C2020A00012: ;
    rdfs:comment "Division 1 Introduction - Abrievated Graph Key: D614"@en-AU ;
    skos:broader C2020A00012:615 ;
    skos:definition "Division 1 Introduction"@en-AU ;
    skos:narrower C2020A00012:613 ;
    skos:prefLabel "Division D614"@en-AU ;
    dcat:accessURL <https://www.legislation.gov.au/C2020A00012/2024-07-10/2024-07-10/text/original/epub/OEBPS/document_1/document_1.html#_Toc172119306> ;
    dcat:landingPage "https://www.legislation.gov.au/C2020A00012/2024-07-10/2024-07-10/text/original/epub/OEBPS/document_1/document_1.html#_Toc172119306"^^xsd:anyURI ;
    dcat:theme legcons:Division .

C2020A00012:616 a legcons:Division,
        owl:Class,
        dcat:Resource ;
    rdfs:label "Division - D616 Division 2 Fees"@en-AU ;
    dct:hasPart C2020A00012:617 ;
    dct:isPartOf C2020A00012:613 ;
    dct:isReferencedBy C2020A00012: ;
    rdfs:comment "Division 2 Fees - Abrievated Graph Key: D616"@en-AU ;
    skos:broader C2020A00012:617 ;
    skos:definition "Division 2 Fees"@en-AU ;
    skos:narrower C2020A00012:613 ;
    skos:prefLabel "Division D616"@en-AU ;
    dcat:accessURL <https://www.legislation.gov.au/C2020A00012/2024-07-10/2024-07-10/text/original/epub/OEBPS/document_1/document_1.html#_Toc172119308> ;
    dcat:landingPage "https://www.legislation.gov.au/C2020A00012/2024-07-10/2024-07-10/text/original/epub/OEBPS/document_1/document_1.html#_Toc172119308"^^xsd:anyURI ;
    dcat:theme legcons:Division .

C2020A00012:629 a legcons:Division,
        owl:Class,
        dcat:Resource ;
    rdfs:label "Division - D629 Division 1 Introduction"@en-AU ;
    dct:hasPart C2020A00012:630 ;
    dct:isPartOf C2020A00012:628 ;
    dct:isReferencedBy C2020A00012: ;
    rdfs:comment "Division 1 Introduction - Abrievated Graph Key: D629"@en-AU ;
    skos:broader C2020A00012:630 ;
    skos:definition "Division 1 Introduction"@en-AU ;
    skos:narrower C2020A00012:628 ;
    skos:prefLabel "Division D629"@en-AU ;
    dcat:accessURL <https://www.legislation.gov.au/C2020A00012/2024-07-10/2024-07-10/text/original/epub/OEBPS/document_1/document_1.html#_Toc172119321> ;
    dcat:landingPage "https://www.legislation.gov.au/C2020A00012/2024-07-10/2024-07-10/text/original/epub/OEBPS/document_1/document_1.html#_Toc172119321"^^xsd:anyURI ;
    dcat:theme legcons:Division .

C2020A00012:631 a legcons:Division,
        owl:Class,
        dcat:Resource ;
    rdfs:label "Division - D631 Division 2 Records"@en-AU ;
    dct:hasPart C2020A00012:632 ;
    dct:isPartOf C2020A00012:628 ;
    dct:isReferencedBy C2020A00012: ;
    rdfs:comment "Division 2 Records - Abrievated Graph Key: D631"@en-AU ;
    skos:broader C2020A00012:632 ;
    skos:definition "Division 2 Records"@en-AU ;
    skos:narrower C2020A00012:628 ;
    skos:prefLabel "Division D631"@en-AU ;
    dcat:accessURL <https://www.legislation.gov.au/C2020A00012/2024-07-10/2024-07-10/text/original/epub/OEBPS/document_1/document_1.html#_Toc172119323> ;
    dcat:landingPage "https://www.legislation.gov.au/C2020A00012/2024-07-10/2024-07-10/text/original/epub/OEBPS/document_1/document_1.html#_Toc172119323"^^xsd:anyURI ;
    dcat:theme legcons:Division .

C2020A00012:634 a legcons:Division,
        owl:Class,
        dcat:Resource ;
    rdfs:label "Division - D634 Division 1 Introduction"@en-AU ;
    dct:hasPart C2020A00012:635 ;
    dct:isPartOf C2020A00012:633 ;
    dct:isReferencedBy C2020A00012: ;
    rdfs:comment "Division 1 Introduction - Abrievated Graph Key: D634"@en-AU ;
    skos:broader C2020A00012:635 ;
    skos:definition "Division 1 Introduction"@en-AU ;
    skos:narrower C2020A00012:633 ;
    skos:prefLabel "Division D634"@en-AU ;
    dcat:accessURL <https://www.legislation.gov.au/C2020A00012/2024-07-10/2024-07-10/text/original/epub/OEBPS/document_1/document_1.html#_Toc172119326> ;
    dcat:landingPage "https://www.legislation.gov.au/C2020A00012/2024-07-10/2024-07-10/text/original/epub/OEBPS/document_1/document_1.html#_Toc172119326"^^xsd:anyURI ;
    dcat:theme legcons:Division .

C2020A00012:643 a legcons:Division,
        owl:Class,
        dcat:Resource ;
    rdfs:label "Division - D643 Division 3 Forfeiture of goods"@en-AU ;
    dct:hasPart C2020A00012:644 ;
    dct:isPartOf C2020A00012:633 ;
    dct:isReferencedBy C2020A00012: ;
    rdfs:comment "Division 3 Forfeiture of goods - Abrievated Graph Key: D643"@en-AU ;
    skos:broader C2020A00012:644 ;
    skos:definition "Division 3 Forfeiture of goods"@en-AU ;
    skos:narrower C2020A00012:633 ;
    skos:prefLabel "Division D643"@en-AU ;
    dcat:accessURL <https://www.legislation.gov.au/C2020A00012/2024-07-10/2024-07-10/text/original/epub/OEBPS/document_1/document_1.html#_Toc172119335> ;
    dcat:landingPage "https://www.legislation.gov.au/C2020A00012/2024-07-10/2024-07-10/text/original/epub/OEBPS/document_1/document_1.html#_Toc172119335"^^xsd:anyURI ;
    dcat:theme legcons:Division .

C2020A00012:654 a legcons:Division,
        owl:Class,
        dcat:Resource ;
    rdfs:label "Division - D654 Division 6 Matters relating to export of livestock"@en-AU ;
    dct:hasPart C2020A00012:655 ;
    dct:isPartOf C2020A00012:633 ;
    dct:isReferencedBy C2020A00012: ;
    rdfs:comment "Division 6 Matters relating to export of livestock - Abrievated Graph Key: D654"@en-AU ;
    skos:broader C2020A00012:655 ;
    skos:definition "Division 6 Matters relating to export of livestock"@en-AU ;
    skos:narrower C2020A00012:633 ;
    skos:prefLabel "Division D654"@en-AU ;
    dcat:accessURL <https://www.legislation.gov.au/C2020A00012/2024-07-10/2024-07-10/text/original/epub/OEBPS/document_1/document_1.html#_Toc172119346> ;
    dcat:landingPage "https://www.legislation.gov.au/C2020A00012/2024-07-10/2024-07-10/text/original/epub/OEBPS/document_1/document_1.html#_Toc172119346"^^xsd:anyURI ;
    dcat:theme legcons:Division .

C2020A00012:80 a legcons:Division,
        owl:Class,
        dcat:Resource ;
    rdfs:label "Division - D80 Division 1 Introduction"@en-AU ;
    dct:hasPart C2020A00012:81 ;
    dct:isPartOf C2020A00012:27 ;
    dct:isReferencedBy C2020A00012: ;
    rdfs:comment "Division 1 Introduction - Abrievated Graph Key: D80"@en-AU ;
    skos:broader C2020A00012:81 ;
    skos:definition "Division 1 Introduction"@en-AU ;
    skos:narrower C2020A00012:27 ;
    skos:prefLabel "Division D80"@en-AU ;
    dcat:accessURL <https://www.legislation.gov.au/C2020A00012/2024-07-10/2024-07-10/text/original/epub/OEBPS/document_1/document_1.html#_Toc172118772> ;
    dcat:landingPage "https://www.legislation.gov.au/C2020A00012/2024-07-10/2024-07-10/text/original/epub/OEBPS/document_1/document_1.html#_Toc172118772"^^xsd:anyURI ;
    dcat:theme legcons:Division .

C2020A00012:114 a legcons:Part,
        owl:Class,
        dcat:Resource ;
    rdfs:label "Part - P114 Part 4 Variation of accreditation"@en-AU ;
    dct:hasPart C2020A00012:115,
        C2020A00012:119 ;
    dct:isPartOf C2020A00012:100 ;
    dct:isReferencedBy C2020A00012: ;
    rdfs:comment "Part 4 Variation of accreditation - Abrievated Graph Key: P114"@en-AU ;
    skos:broader C2020A00012:115,
        C2020A00012:119 ;
    skos:definition "Part 4 Variation of accreditation"@en-AU ;
    skos:narrower C2020A00012:100 ;
    skos:prefLabel "Part P114"@en-AU ;
    dcat:accessURL <https://www.legislation.gov.au/C2020A00012/2024-07-10/2024-07-10/text/original/epub/OEBPS/document_1/document_1.html#_Toc172118806> ;
    dcat:landingPage "https://www.legislation.gov.au/C2020A00012/2024-07-10/2024-07-10/text/original/epub/OEBPS/document_1/document_1.html#_Toc172118806"^^xsd:anyURI ;
    dcat:theme legcons:Part .

C2020A00012:119 a legcons:Division,
        owl:Class,
        dcat:Resource ;
    rdfs:label "Division - D119 Division 2 Variation by Secretary"@en-AU ;
    dct:hasPart C2020A00012:120,
        C2020A00012:121 ;
    dct:isPartOf C2020A00012:114 ;
    dct:isReferencedBy C2020A00012: ;
    rdfs:comment "Division 2 Variation by Secretary - Abrievated Graph Key: D119"@en-AU ;
    skos:broader C2020A00012:120,
        C2020A00012:121 ;
    skos:definition "Division 2 Variation by Secretary"@en-AU ;
    skos:narrower C2020A00012:114 ;
    skos:prefLabel "Division D119"@en-AU ;
    dcat:accessURL <https://www.legislation.gov.au/C2020A00012/2024-07-10/2024-07-10/text/original/epub/OEBPS/document_1/document_1.html#_Toc172118811> ;
    dcat:landingPage "https://www.legislation.gov.au/C2020A00012/2024-07-10/2024-07-10/text/original/epub/OEBPS/document_1/document_1.html#_Toc172118811"^^xsd:anyURI ;
    dcat:theme legcons:Division .

C2020A00012:123 a legcons:Division,
        owl:Class,
        dcat:Resource ;
    rdfs:label "Division - D123 Division 1 Suspension requested by manager"@en-AU ;
    dct:hasPart C2020A00012:124,
        C2020A00012:125 ;
    dct:isPartOf C2020A00012:122 ;
    dct:isReferencedBy C2020A00012: ;
    rdfs:comment "Division 1 Suspension requested by manager - Abrievated Graph Key: D123"@en-AU ;
    skos:broader C2020A00012:124,
        C2020A00012:125 ;
    skos:definition "Division 1 Suspension requested by manager"@en-AU ;
    skos:narrower C2020A00012:122 ;
    skos:prefLabel "Division D123"@en-AU ;
    dcat:accessURL <https://www.legislation.gov.au/C2020A00012/2024-07-10/2024-07-10/text/original/epub/OEBPS/document_1/document_1.html#_Toc172118815> ;
    dcat:landingPage "https://www.legislation.gov.au/C2020A00012/2024-07-10/2024-07-10/text/original/epub/OEBPS/document_1/document_1.html#_Toc172118815"^^xsd:anyURI ;
    dcat:theme legcons:Division .

C2020A00012:132 a legcons:Division,
        owl:Class,
        dcat:Resource ;
    rdfs:label "Division - D132 Division 3 Other provisions"@en-AU ;
    dct:hasPart C2020A00012:133,
        C2020A00012:134 ;
    dct:isPartOf C2020A00012:122 ;
    dct:isReferencedBy C2020A00012: ;
    rdfs:comment "Division 3 Other provisions - Abrievated Graph Key: D132"@en-AU ;
    skos:broader C2020A00012:133,
        C2020A00012:134 ;
    skos:definition "Division 3 Other provisions"@en-AU ;
    skos:narrower C2020A00012:122 ;
    skos:prefLabel "Division D132"@en-AU ;
    dcat:accessURL <https://www.legislation.gov.au/C2020A00012/2024-07-10/2024-07-10/text/original/epub/OEBPS/document_1/document_1.html#_Toc172118824> ;
    dcat:landingPage "https://www.legislation.gov.au/C2020A00012/2024-07-10/2024-07-10/text/original/epub/OEBPS/document_1/document_1.html#_Toc172118824"^^xsd:anyURI ;
    dcat:theme legcons:Division .

C2020A00012:163 a legcons:Part,
        owl:Class,
        dcat:Resource ;
    rdfs:label "Part - P163 Part 4 Variation of registration"@en-AU ;
    dct:hasPart C2020A00012:164,
        C2020A00012:168 ;
    dct:isPartOf C2020A00012:149 ;
    dct:isReferencedBy C2020A00012: ;
    rdfs:comment "Part 4 Variation of registration - Abrievated Graph Key: P163"@en-AU ;
    skos:broader C2020A00012:164,
        C2020A00012:168 ;
    skos:definition "Part 4 Variation of registration"@en-AU ;
    skos:narrower C2020A00012:149 ;
    skos:prefLabel "Part P163"@en-AU ;
    dcat:accessURL <https://www.legislation.gov.au/C2020A00012/2024-07-10/2024-07-10/text/original/epub/OEBPS/document_1/document_1.html#_Toc172118855> ;
    dcat:landingPage "https://www.legislation.gov.au/C2020A00012/2024-07-10/2024-07-10/text/original/epub/OEBPS/document_1/document_1.html#_Toc172118855"^^xsd:anyURI ;
    dcat:theme legcons:Part .

C2020A00012:168 a legcons:Division,
        owl:Class,
        dcat:Resource ;
    rdfs:label "Division - D168 Division 2 Variation by Secretary"@en-AU ;
    dct:hasPart C2020A00012:169,
        C2020A00012:170 ;
    dct:isPartOf C2020A00012:163 ;
    dct:isReferencedBy C2020A00012: ;
    rdfs:comment "Division 2 Variation by Secretary - Abrievated Graph Key: D168"@en-AU ;
    skos:broader C2020A00012:169,
        C2020A00012:170 ;
    skos:definition "Division 2 Variation by Secretary"@en-AU ;
    skos:narrower C2020A00012:163 ;
    skos:prefLabel "Division D168"@en-AU ;
    dcat:accessURL <https://www.legislation.gov.au/C2020A00012/2024-07-10/2024-07-10/text/original/epub/OEBPS/document_1/document_1.html#_Toc172118860> ;
    dcat:landingPage "https://www.legislation.gov.au/C2020A00012/2024-07-10/2024-07-10/text/original/epub/OEBPS/document_1/document_1.html#_Toc172118860"^^xsd:anyURI ;
    dcat:theme legcons:Division .

C2020A00012:172 a legcons:Division,
        owl:Class,
        dcat:Resource ;
    rdfs:label "Division - D172 Division 1 Suspension requested by occupier"@en-AU ;
    dct:hasPart C2020A00012:173,
        C2020A00012:174 ;
    dct:isPartOf C2020A00012:171 ;
    dct:isReferencedBy C2020A00012: ;
    rdfs:comment "Division 1 Suspension requested by occupier - Abrievated Graph Key: D172"@en-AU ;
    skos:broader C2020A00012:173,
        C2020A00012:174 ;
    skos:definition "Division 1 Suspension requested by occupier"@en-AU ;
    skos:narrower C2020A00012:171 ;
    skos:prefLabel "Division D172"@en-AU ;
    dcat:accessURL <https://www.legislation.gov.au/C2020A00012/2024-07-10/2024-07-10/text/original/epub/OEBPS/document_1/document_1.html#_Toc172118864> ;
    dcat:landingPage "https://www.legislation.gov.au/C2020A00012/2024-07-10/2024-07-10/text/original/epub/OEBPS/document_1/document_1.html#_Toc172118864"^^xsd:anyURI ;
    dcat:theme legcons:Division .

C2020A00012:185 a legcons:Division,
        owl:Class,
        dcat:Resource ;
    rdfs:label "Division - D185 Division 4 Other provisions"@en-AU ;
    dct:hasPart C2020A00012:186,
        C2020A00012:187 ;
    dct:isPartOf C2020A00012:171 ;
    dct:isReferencedBy C2020A00012: ;
    rdfs:comment "Division 4 Other provisions - Abrievated Graph Key: D185"@en-AU ;
    skos:broader C2020A00012:186,
        C2020A00012:187 ;
    skos:definition "Division 4 Other provisions"@en-AU ;
    skos:narrower C2020A00012:171 ;
    skos:prefLabel "Division D185"@en-AU ;
    dcat:accessURL <https://www.legislation.gov.au/C2020A00012/2024-07-10/2024-07-10/text/original/epub/OEBPS/document_1/document_1.html#_Toc172118877> ;
    dcat:landingPage "https://www.legislation.gov.au/C2020A00012/2024-07-10/2024-07-10/text/original/epub/OEBPS/document_1/document_1.html#_Toc172118877"^^xsd:anyURI ;
    dcat:theme legcons:Division .

C2020A00012:195 a legcons:Division,
        owl:Class,
        dcat:Resource ;
    rdfs:label "Division - D195 Division 3 Other provisions"@en-AU ;
    dct:hasPart C2020A00012:196,
        C2020A00012:197 ;
    dct:isPartOf C2020A00012:188 ;
    dct:isReferencedBy C2020A00012: ;
    rdfs:comment "Division 3 Other provisions - Abrievated Graph Key: D195"@en-AU ;
    skos:broader C2020A00012:196,
        C2020A00012:197 ;
    skos:definition "Division 3 Other provisions"@en-AU ;
    skos:narrower C2020A00012:188 ;
    skos:prefLabel "Division D195"@en-AU ;
    dcat:accessURL <https://www.legislation.gov.au/C2020A00012/2024-07-10/2024-07-10/text/original/epub/OEBPS/document_1/document_1.html#_Toc172118887> ;
    dcat:landingPage "https://www.legislation.gov.au/C2020A00012/2024-07-10/2024-07-10/text/original/epub/OEBPS/document_1/document_1.html#_Toc172118887"^^xsd:anyURI ;
    dcat:theme legcons:Division .

C2020A00012:220 a legcons:Part,
        owl:Class,
        dcat:Resource ;
    rdfs:label "Part - P220 Part 4 Variation of approved arrangement"@en-AU ;
    dct:hasPart C2020A00012:221,
        C2020A00012:231 ;
    dct:isPartOf C2020A00012:206 ;
    dct:isReferencedBy C2020A00012: ;
    rdfs:comment "Part 4 Variation of approved arrangement - Abrievated Graph Key: P220"@en-AU ;
    skos:broader C2020A00012:221,
        C2020A00012:231 ;
    skos:definition "Part 4 Variation of approved arrangement"@en-AU ;
    skos:narrower C2020A00012:206 ;
    skos:prefLabel "Part P220"@en-AU ;
    dcat:accessURL <https://www.legislation.gov.au/C2020A00012/2024-07-10/2024-07-10/text/original/epub/OEBPS/document_1/document_1.html#_Toc172118912> ;
    dcat:landingPage "https://www.legislation.gov.au/C2020A00012/2024-07-10/2024-07-10/text/original/epub/OEBPS/document_1/document_1.html#_Toc172118912"^^xsd:anyURI ;
    dcat:theme legcons:Part .

C2020A00012:222 a legcons:Subdivision,
        owl:Class,
        dcat:Resource ;
    rdfs:label "Subdivision - S222 Subdivision ANon significant variations"@en-AU ;
    dct:hasPart C2020A00012:223,
        C2020A00012:224 ;
    dct:isPartOf C2020A00012:221 ;
    dct:isReferencedBy C2020A00012: ;
    rdfs:comment "Subdivision ANon significant variations - Abrievated Graph Key: S222"@en-AU ;
    skos:broader C2020A00012:223,
        C2020A00012:224 ;
    skos:definition "Subdivision ANon significant variations"@en-AU ;
    skos:narrower C2020A00012:221 ;
    skos:prefLabel "Subdivision S222"@en-AU ;
    dcat:accessURL <https://www.legislation.gov.au/C2020A00012/2024-07-10/2024-07-10/text/original/epub/OEBPS/document_1/document_1.html#_Toc172118914> ;
    dcat:landingPage "https://www.legislation.gov.au/C2020A00012/2024-07-10/2024-07-10/text/original/epub/OEBPS/document_1/document_1.html#_Toc172118914"^^xsd:anyURI ;
    dcat:theme legcons:Subdivision .

C2020A00012:237 a legcons:Division,
        owl:Class,
        dcat:Resource ;
    rdfs:label "Division - D237 Division 1 Suspension requested by holder"@en-AU ;
    dct:hasPart C2020A00012:238,
        C2020A00012:239 ;
    dct:isPartOf C2020A00012:236 ;
    dct:isReferencedBy C2020A00012: ;
    rdfs:comment "Division 1 Suspension requested by holder - Abrievated Graph Key: D237"@en-AU ;
    skos:broader C2020A00012:238,
        C2020A00012:239 ;
    skos:definition "Division 1 Suspension requested by holder"@en-AU ;
    skos:narrower C2020A00012:236 ;
    skos:prefLabel "Division D237"@en-AU ;
    dcat:accessURL <https://www.legislation.gov.au/C2020A00012/2024-07-10/2024-07-10/text/original/epub/OEBPS/document_1/document_1.html#_Toc172118929> ;
    dcat:landingPage "https://www.legislation.gov.au/C2020A00012/2024-07-10/2024-07-10/text/original/epub/OEBPS/document_1/document_1.html#_Toc172118929"^^xsd:anyURI ;
    dcat:theme legcons:Division .

C2020A00012:246 a legcons:Division,
        owl:Class,
        dcat:Resource ;
    rdfs:label "Division - D246 Division 3 Other provisions"@en-AU ;
    dct:hasPart C2020A00012:247,
        C2020A00012:248 ;
    dct:isPartOf C2020A00012:236 ;
    dct:isReferencedBy C2020A00012: ;
    rdfs:comment "Division 3 Other provisions - Abrievated Graph Key: D246"@en-AU ;
    skos:broader C2020A00012:247,
        C2020A00012:248 ;
    skos:definition "Division 3 Other provisions"@en-AU ;
    skos:narrower C2020A00012:236 ;
    skos:prefLabel "Division D246"@en-AU ;
    dcat:accessURL <https://www.legislation.gov.au/C2020A00012/2024-07-10/2024-07-10/text/original/epub/OEBPS/document_1/document_1.html#_Toc172118938> ;
    dcat:landingPage "https://www.legislation.gov.au/C2020A00012/2024-07-10/2024-07-10/text/original/epub/OEBPS/document_1/document_1.html#_Toc172118938"^^xsd:anyURI ;
    dcat:theme legcons:Division .

C2020A00012:256 a legcons:Division,
        owl:Class,
        dcat:Resource ;
    rdfs:label "Division - D256 Division 3 Other provisions"@en-AU ;
    dct:hasPart C2020A00012:257,
        C2020A00012:258 ;
    dct:isPartOf C2020A00012:249 ;
    dct:isReferencedBy C2020A00012: ;
    rdfs:comment "Division 3 Other provisions - Abrievated Graph Key: D256"@en-AU ;
    skos:broader C2020A00012:257,
        C2020A00012:258 ;
    skos:definition "Division 3 Other provisions"@en-AU ;
    skos:narrower C2020A00012:249 ;
    skos:prefLabel "Division D256"@en-AU ;
    dcat:accessURL <https://www.legislation.gov.au/C2020A00012/2024-07-10/2024-07-10/text/original/epub/OEBPS/document_1/document_1.html#_Toc172118948> ;
    dcat:landingPage "https://www.legislation.gov.au/C2020A00012/2024-07-10/2024-07-10/text/original/epub/OEBPS/document_1/document_1.html#_Toc172118948"^^xsd:anyURI ;
    dcat:theme legcons:Division .

C2020A00012:279 a legcons:Part,
        owl:Class,
        dcat:Resource ;
    rdfs:label "Part - P279 Part 4 Variation of export licence"@en-AU ;
    dct:hasPart C2020A00012:280,
        C2020A00012:283 ;
    dct:isPartOf C2020A00012:265 ;
    dct:isReferencedBy C2020A00012: ;
    rdfs:comment "Part 4 Variation of export licence - Abrievated Graph Key: P279"@en-AU ;
    skos:broader C2020A00012:280,
        C2020A00012:283 ;
    skos:definition "Part 4 Variation of export licence"@en-AU ;
    skos:narrower C2020A00012:265 ;
    skos:prefLabel "Part P279"@en-AU ;
    dcat:accessURL <https://www.legislation.gov.au/C2020A00012/2024-07-10/2024-07-10/text/original/epub/OEBPS/document_1/document_1.html#_Toc172118971> ;
    dcat:landingPage "https://www.legislation.gov.au/C2020A00012/2024-07-10/2024-07-10/text/original/epub/OEBPS/document_1/document_1.html#_Toc172118971"^^xsd:anyURI ;
    dcat:theme legcons:Part .

C2020A00012:280 a legcons:Division,
        owl:Class,
        dcat:Resource ;
    rdfs:label "Division - D280 Division 1 Application by holder"@en-AU ;
    dct:hasPart C2020A00012:281,
        C2020A00012:282 ;
    dct:isPartOf C2020A00012:279 ;
    dct:isReferencedBy C2020A00012: ;
    rdfs:comment "Division 1 Application by holder - Abrievated Graph Key: D280"@en-AU ;
    skos:broader C2020A00012:281,
        C2020A00012:282 ;
    skos:definition "Division 1 Application by holder"@en-AU ;
    skos:narrower C2020A00012:279 ;
    skos:prefLabel "Division D280"@en-AU ;
    dcat:accessURL <https://www.legislation.gov.au/C2020A00012/2024-07-10/2024-07-10/text/original/epub/OEBPS/document_1/document_1.html#_Toc172118972> ;
    dcat:landingPage "https://www.legislation.gov.au/C2020A00012/2024-07-10/2024-07-10/text/original/epub/OEBPS/document_1/document_1.html#_Toc172118972"^^xsd:anyURI ;
    dcat:theme legcons:Division .

C2020A00012:283 a legcons:Division,
        owl:Class,
        dcat:Resource ;
    rdfs:label "Division - D283 Division 2 Variation by Secretary"@en-AU ;
    dct:hasPart C2020A00012:284,
        C2020A00012:285 ;
    dct:isPartOf C2020A00012:279 ;
    dct:isReferencedBy C2020A00012: ;
    rdfs:comment "Division 2 Variation by Secretary - Abrievated Graph Key: D283"@en-AU ;
    skos:broader C2020A00012:284,
        C2020A00012:285 ;
    skos:definition "Division 2 Variation by Secretary"@en-AU ;
    skos:narrower C2020A00012:279 ;
    skos:prefLabel "Division D283"@en-AU ;
    dcat:accessURL <https://www.legislation.gov.au/C2020A00012/2024-07-10/2024-07-10/text/original/epub/OEBPS/document_1/document_1.html#_Toc172118975> ;
    dcat:landingPage "https://www.legislation.gov.au/C2020A00012/2024-07-10/2024-07-10/text/original/epub/OEBPS/document_1/document_1.html#_Toc172118975"^^xsd:anyURI ;
    dcat:theme legcons:Division .

C2020A00012:287 a legcons:Division,
        owl:Class,
        dcat:Resource ;
    rdfs:label "Division - D287 Division 1 Suspension requested by holder"@en-AU ;
    dct:hasPart C2020A00012:288,
        C2020A00012:289 ;
    dct:isPartOf C2020A00012:286 ;
    dct:isReferencedBy C2020A00012: ;
    rdfs:comment "Division 1 Suspension requested by holder - Abrievated Graph Key: D287"@en-AU ;
    skos:broader C2020A00012:288,
        C2020A00012:289 ;
    skos:definition "Division 1 Suspension requested by holder"@en-AU ;
    skos:narrower C2020A00012:286 ;
    skos:prefLabel "Division D287"@en-AU ;
    dcat:accessURL <https://www.legislation.gov.au/C2020A00012/2024-07-10/2024-07-10/text/original/epub/OEBPS/document_1/document_1.html#_Toc172118979> ;
    dcat:landingPage "https://www.legislation.gov.au/C2020A00012/2024-07-10/2024-07-10/text/original/epub/OEBPS/document_1/document_1.html#_Toc172118979"^^xsd:anyURI ;
    dcat:theme legcons:Division .

C2020A00012:305 a legcons:Division,
        owl:Class,
        dcat:Resource ;
    rdfs:label "Division - D305 Division 3 Other provisions"@en-AU ;
    dct:hasPart C2020A00012:306,
        C2020A00012:307 ;
    dct:isPartOf C2020A00012:298 ;
    dct:isReferencedBy C2020A00012: ;
    rdfs:comment "Division 3 Other provisions - Abrievated Graph Key: D305"@en-AU ;
    skos:broader C2020A00012:306,
        C2020A00012:307 ;
    skos:definition "Division 3 Other provisions"@en-AU ;
    skos:narrower C2020A00012:298 ;
    skos:prefLabel "Division D305"@en-AU ;
    dcat:accessURL <https://www.legislation.gov.au/C2020A00012/2024-07-10/2024-07-10/text/original/epub/OEBPS/document_1/document_1.html#_Toc172118997> ;
    dcat:landingPage "https://www.legislation.gov.au/C2020A00012/2024-07-10/2024-07-10/text/original/epub/OEBPS/document_1/document_1.html#_Toc172118997"^^xsd:anyURI ;
    dcat:theme legcons:Division .

C2020A00012:32 a legcons:Subdivision,
        owl:Class,
        dcat:Resource ;
    rdfs:label "Subdivision - S32 Subdivision APermanently prohibited goods and exports"@en-AU ;
    dct:hasPart C2020A00012:33,
        C2020A00012:34 ;
    dct:isPartOf C2020A00012:31 ;
    dct:isReferencedBy C2020A00012: ;
    rdfs:comment "Subdivision APermanently prohibited goods and exports - Abrievated Graph Key: S32"@en-AU ;
    skos:broader C2020A00012:33,
        C2020A00012:34 ;
    skos:definition "Subdivision APermanently prohibited goods and exports"@en-AU ;
    skos:narrower C2020A00012:31 ;
    skos:prefLabel "Subdivision S32"@en-AU ;
    dcat:accessURL <https://www.legislation.gov.au/C2020A00012/2024-07-10/2024-07-10/text/original/epub/OEBPS/document_1/document_1.html#_Toc172118724> ;
    dcat:landingPage "https://www.legislation.gov.au/C2020A00012/2024-07-10/2024-07-10/text/original/epub/OEBPS/document_1/document_1.html#_Toc172118724"^^xsd:anyURI ;
    dcat:theme legcons:Subdivision .

C2020A00012:342 a legcons:Part,
        owl:Class,
        dcat:Resource ;
    rdfs:label "Part - P342 Part 1 Notices of intention to export"@en-AU ;
    dct:hasPart C2020A00012:343,
        C2020A00012:345 ;
    dct:isPartOf C2020A00012:341 ;
    dct:isReferencedBy C2020A00012: ;
    rdfs:comment "Part 1 Notices of intention to export - Abrievated Graph Key: P342"@en-AU ;
    skos:broader C2020A00012:343,
        C2020A00012:345 ;
    skos:definition "Part 1 Notices of intention to export"@en-AU ;
    skos:narrower C2020A00012:341 ;
    skos:prefLabel "Part P342"@en-AU ;
    dcat:accessURL <https://www.legislation.gov.au/C2020A00012/2024-07-10/2024-07-10/text/original/epub/OEBPS/document_1/document_1.html#_Toc172119034> ;
    dcat:landingPage "https://www.legislation.gov.au/C2020A00012/2024-07-10/2024-07-10/text/original/epub/OEBPS/document_1/document_1.html#_Toc172119034"^^xsd:anyURI ;
    dcat:theme legcons:Part .

C2020A00012:345 a legcons:Division,
        owl:Class,
        dcat:Resource ;
    rdfs:label "Division - D345 Division 2 Notices of intention to export"@en-AU ;
    dct:hasPart C2020A00012:346,
        C2020A00012:347 ;
    dct:isPartOf C2020A00012:342 ;
    dct:isReferencedBy C2020A00012: ;
    rdfs:comment "Division 2 Notices of intention to export - Abrievated Graph Key: D345"@en-AU ;
    skos:broader C2020A00012:346,
        C2020A00012:347 ;
    skos:definition "Division 2 Notices of intention to export"@en-AU ;
    skos:narrower C2020A00012:342 ;
    skos:prefLabel "Division D345"@en-AU ;
    dcat:accessURL <https://www.legislation.gov.au/C2020A00012/2024-07-10/2024-07-10/text/original/epub/OEBPS/document_1/document_1.html#_Toc172119037> ;
    dcat:landingPage "https://www.legislation.gov.au/C2020A00012/2024-07-10/2024-07-10/text/original/epub/OEBPS/document_1/document_1.html#_Toc172119037"^^xsd:anyURI ;
    dcat:theme legcons:Division .

C2020A00012:374 a legcons:Part,
        owl:Class,
        dcat:Resource ;
    rdfs:label "Part - P374 Part 4 Tariff rate quotas"@en-AU ;
    dct:hasPart C2020A00012:375,
        C2020A00012:377 ;
    dct:isPartOf C2020A00012:341 ;
    dct:isReferencedBy C2020A00012: ;
    rdfs:comment "Part 4 Tariff rate quotas - Abrievated Graph Key: P374"@en-AU ;
    skos:broader C2020A00012:375,
        C2020A00012:377 ;
    skos:definition "Part 4 Tariff rate quotas"@en-AU ;
    skos:narrower C2020A00012:341 ;
    skos:prefLabel "Part P374"@en-AU ;
    dcat:accessURL <https://www.legislation.gov.au/C2020A00012/2024-07-10/2024-07-10/text/original/epub/OEBPS/document_1/document_1.html#_Toc172119066> ;
    dcat:landingPage "https://www.legislation.gov.au/C2020A00012/2024-07-10/2024-07-10/text/original/epub/OEBPS/document_1/document_1.html#_Toc172119066"^^xsd:anyURI ;
    dcat:theme legcons:Part .

C2020A00012:407 a legcons:Part,
        owl:Class,
        dcat:Resource ;
    rdfs:label "Part - P407 Part 3 Powers of the Secretary"@en-AU ;
    dct:hasPart C2020A00012:408,
        C2020A00012:410 ;
    dct:isPartOf C2020A00012:379 ;
    dct:isReferencedBy C2020A00012: ;
    rdfs:comment "Part 3 Powers of the Secretary - Abrievated Graph Key: P407"@en-AU ;
    skos:broader C2020A00012:408,
        C2020A00012:410 ;
    skos:definition "Part 3 Powers of the Secretary"@en-AU ;
    skos:narrower C2020A00012:379 ;
    skos:prefLabel "Part P407"@en-AU ;
    dcat:accessURL <https://www.legislation.gov.au/C2020A00012/2024-07-10/2024-07-10/text/original/epub/OEBPS/document_1/document_1.html#_Toc172119099> ;
    dcat:landingPage "https://www.legislation.gov.au/C2020A00012/2024-07-10/2024-07-10/text/original/epub/OEBPS/document_1/document_1.html#_Toc172119099"^^xsd:anyURI ;
    dcat:theme legcons:Part .

C2020A00012:468 a legcons:Part,
        owl:Class,
        dcat:Resource ;
    rdfs:label "Part - P468 Part 1 Introduction"@en-AU ;
    dct:hasPart C2020A00012:469,
        C2020A00012:470 ;
    dct:isPartOf C2020A00012:467 ;
    dct:isReferencedBy C2020A00012: ;
    rdfs:comment "Part 1 Introduction - Abrievated Graph Key: P468"@en-AU ;
    skos:broader C2020A00012:469,
        C2020A00012:470 ;
    skos:definition "Part 1 Introduction"@en-AU ;
    skos:narrower C2020A00012:467 ;
    skos:prefLabel "Part P468"@en-AU ;
    dcat:accessURL <https://www.legislation.gov.au/C2020A00012/2024-07-10/2024-07-10/text/original/epub/OEBPS/document_1/document_1.html#_Toc172119160> ;
    dcat:landingPage "https://www.legislation.gov.au/C2020A00012/2024-07-10/2024-07-10/text/original/epub/OEBPS/document_1/document_1.html#_Toc172119160"^^xsd:anyURI ;
    dcat:theme legcons:Part .

C2020A00012:471 a legcons:Part,
        owl:Class,
        dcat:Resource ;
    rdfs:label "Part - P471 Part 2 Monitoring"@en-AU ;
    dct:hasPart C2020A00012:472,
        C2020A00012:474 ;
    dct:isPartOf C2020A00012:467 ;
    dct:isReferencedBy C2020A00012: ;
    rdfs:comment "Part 2 Monitoring - Abrievated Graph Key: P471"@en-AU ;
    skos:broader C2020A00012:472,
        C2020A00012:474 ;
    skos:definition "Part 2 Monitoring"@en-AU ;
    skos:narrower C2020A00012:467 ;
    skos:prefLabel "Part P471"@en-AU ;
    dcat:accessURL <https://www.legislation.gov.au/C2020A00012/2024-07-10/2024-07-10/text/original/epub/OEBPS/document_1/document_1.html#_Toc172119163> ;
    dcat:landingPage "https://www.legislation.gov.au/C2020A00012/2024-07-10/2024-07-10/text/original/epub/OEBPS/document_1/document_1.html#_Toc172119163"^^xsd:anyURI ;
    dcat:theme legcons:Part .

C2020A00012:474 a legcons:Division,
        owl:Class,
        dcat:Resource ;
    rdfs:label "Division - D474 Division 2 Monitoring under Part 2 of the Regulatory Powers Act"@en-AU ;
    dct:hasPart C2020A00012:475,
        C2020A00012:476 ;
    dct:isPartOf C2020A00012:471 ;
    dct:isReferencedBy C2020A00012: ;
    rdfs:comment "Division 2 Monitoring under Part 2 of the Regulatory Powers Act - Abrievated Graph Key: D474"@en-AU ;
    skos:broader C2020A00012:475,
        C2020A00012:476 ;
    skos:definition "Division 2 Monitoring under Part 2 of the Regulatory Powers Act"@en-AU ;
    skos:narrower C2020A00012:471 ;
    skos:prefLabel "Division D474"@en-AU ;
    dcat:accessURL <https://www.legislation.gov.au/C2020A00012/2024-07-10/2024-07-10/text/original/epub/OEBPS/document_1/document_1.html#_Toc172119166> ;
    dcat:landingPage "https://www.legislation.gov.au/C2020A00012/2024-07-10/2024-07-10/text/original/epub/OEBPS/document_1/document_1.html#_Toc172119166"^^xsd:anyURI ;
    dcat:theme legcons:Division .

C2020A00012:477 a legcons:Part,
        owl:Class,
        dcat:Resource ;
    rdfs:label "Part - P477 Part 3 Investigation"@en-AU ;
    dct:hasPart C2020A00012:478,
        C2020A00012:480 ;
    dct:isPartOf C2020A00012:467 ;
    dct:isReferencedBy C2020A00012: ;
    rdfs:comment "Part 3 Investigation - Abrievated Graph Key: P477"@en-AU ;
    skos:broader C2020A00012:478,
        C2020A00012:480 ;
    skos:definition "Part 3 Investigation"@en-AU ;
    skos:narrower C2020A00012:467 ;
    skos:prefLabel "Part P477"@en-AU ;
    dcat:accessURL <https://www.legislation.gov.au/C2020A00012/2024-07-10/2024-07-10/text/original/epub/OEBPS/document_1/document_1.html#_Toc172119169> ;
    dcat:landingPage "https://www.legislation.gov.au/C2020A00012/2024-07-10/2024-07-10/text/original/epub/OEBPS/document_1/document_1.html#_Toc172119169"^^xsd:anyURI ;
    dcat:theme legcons:Part .

C2020A00012:480 a legcons:Division,
        owl:Class,
        dcat:Resource ;
    rdfs:label "Division - D480 Division 2 Investigating under Part 3 of the Regulatory Powers Act"@en-AU ;
    dct:hasPart C2020A00012:481,
        C2020A00012:482 ;
    dct:isPartOf C2020A00012:477 ;
    dct:isReferencedBy C2020A00012: ;
    rdfs:comment "Division 2 Investigating under Part 3 of the Regulatory Powers Act - Abrievated Graph Key: D480"@en-AU ;
    skos:broader C2020A00012:481,
        C2020A00012:482 ;
    skos:definition "Division 2 Investigating under Part 3 of the Regulatory Powers Act"@en-AU ;
    skos:narrower C2020A00012:477 ;
    skos:prefLabel "Division D480"@en-AU ;
    dcat:accessURL <https://www.legislation.gov.au/C2020A00012/2024-07-10/2024-07-10/text/original/epub/OEBPS/document_1/document_1.html#_Toc172119172> ;
    dcat:landingPage "https://www.legislation.gov.au/C2020A00012/2024-07-10/2024-07-10/text/original/epub/OEBPS/document_1/document_1.html#_Toc172119172"^^xsd:anyURI ;
    dcat:theme legcons:Division .

C2020A00012:484 a legcons:Division,
        owl:Class,
        dcat:Resource ;
    rdfs:label "Division - D484 Division 1 Introduction"@en-AU ;
    dct:hasPart C2020A00012:485,
        C2020A00012:486 ;
    dct:isPartOf C2020A00012:483 ;
    dct:isReferencedBy C2020A00012: ;
    rdfs:comment "Division 1 Introduction - Abrievated Graph Key: D484"@en-AU ;
    skos:broader C2020A00012:485,
        C2020A00012:486 ;
    skos:definition "Division 1 Introduction"@en-AU ;
    skos:narrower C2020A00012:483 ;
    skos:prefLabel "Division D484"@en-AU ;
    dcat:accessURL <https://www.legislation.gov.au/C2020A00012/2024-07-10/2024-07-10/text/original/epub/OEBPS/document_1/document_1.html#_Toc172119176> ;
    dcat:landingPage "https://www.legislation.gov.au/C2020A00012/2024-07-10/2024-07-10/text/original/epub/OEBPS/document_1/document_1.html#_Toc172119176"^^xsd:anyURI ;
    dcat:theme legcons:Division .

C2020A00012:487 a legcons:Division,
        owl:Class,
        dcat:Resource ;
    rdfs:label "Division - D487 Division 2 Entering adjacent premises to gain access to other premises"@en-AU ;
    dct:hasPart C2020A00012:488,
        C2020A00012:489 ;
    dct:isPartOf C2020A00012:483 ;
    dct:isReferencedBy C2020A00012: ;
    rdfs:comment "Division 2 Entering adjacent premises to gain access to other premises - Abrievated Graph Key: D487"@en-AU ;
    skos:broader C2020A00012:488,
        C2020A00012:489 ;
    skos:definition "Division 2 Entering adjacent premises to gain access to other premises"@en-AU ;
    skos:narrower C2020A00012:483 ;
    skos:prefLabel "Division D487"@en-AU ;
    dcat:accessURL <https://www.legislation.gov.au/C2020A00012/2024-07-10/2024-07-10/text/original/epub/OEBPS/document_1/document_1.html#_Toc172119179> ;
    dcat:landingPage "https://www.legislation.gov.au/C2020A00012/2024-07-10/2024-07-10/text/original/epub/OEBPS/document_1/document_1.html#_Toc172119179"^^xsd:anyURI ;
    dcat:theme legcons:Division .

C2020A00012:498 a legcons:Division,
        owl:Class,
        dcat:Resource ;
    rdfs:label "Division - D498 Division 5 Appropriate persons rights and responsibilities"@en-AU ;
    dct:hasPart C2020A00012:499,
        C2020A00012:500 ;
    dct:isPartOf C2020A00012:483 ;
    dct:isReferencedBy C2020A00012: ;
    rdfs:comment "Division 5 Appropriate persons rights and responsibilities - Abrievated Graph Key: D498"@en-AU ;
    skos:broader C2020A00012:499,
        C2020A00012:500 ;
    skos:definition "Division 5 Appropriate persons rights and responsibilities"@en-AU ;
    skos:narrower C2020A00012:483 ;
    skos:prefLabel "Division D498"@en-AU ;
    dcat:accessURL <https://www.legislation.gov.au/C2020A00012/2024-07-10/2024-07-10/text/original/epub/OEBPS/document_1/document_1.html#_Toc172119190> ;
    dcat:landingPage "https://www.legislation.gov.au/C2020A00012/2024-07-10/2024-07-10/text/original/epub/OEBPS/document_1/document_1.html#_Toc172119190"^^xsd:anyURI ;
    dcat:theme legcons:Division .

C2020A00012:504 a legcons:Division,
        owl:Class,
        dcat:Resource ;
    rdfs:label "Division - D504 Division 1 Introduction"@en-AU ;
    dct:hasPart C2020A00012:505,
        C2020A00012:506 ;
    dct:isPartOf C2020A00012:503 ;
    dct:isReferencedBy C2020A00012: ;
    rdfs:comment "Division 1 Introduction - Abrievated Graph Key: D504"@en-AU ;
    skos:broader C2020A00012:505,
        C2020A00012:506 ;
    skos:definition "Division 1 Introduction"@en-AU ;
    skos:narrower C2020A00012:503 ;
    skos:prefLabel "Division D504"@en-AU ;
    dcat:accessURL <https://www.legislation.gov.au/C2020A00012/2024-07-10/2024-07-10/text/original/epub/OEBPS/document_1/document_1.html#_Toc172119196> ;
    dcat:landingPage "https://www.legislation.gov.au/C2020A00012/2024-07-10/2024-07-10/text/original/epub/OEBPS/document_1/document_1.html#_Toc172119196"^^xsd:anyURI ;
    dcat:theme legcons:Division .

C2020A00012:507 a legcons:Division,
        owl:Class,
        dcat:Resource ;
    rdfs:label "Division - D507 Division 2 Monitoring and searching relevant premises"@en-AU ;
    dct:hasPart C2020A00012:508,
        C2020A00012:509 ;
    dct:isPartOf C2020A00012:503 ;
    dct:isReferencedBy C2020A00012: ;
    rdfs:comment "Division 2 Monitoring and searching relevant premises - Abrievated Graph Key: D507"@en-AU ;
    skos:broader C2020A00012:508,
        C2020A00012:509 ;
    skos:definition "Division 2 Monitoring and searching relevant premises"@en-AU ;
    skos:narrower C2020A00012:503 ;
    skos:prefLabel "Division D507"@en-AU ;
    dcat:accessURL <https://www.legislation.gov.au/C2020A00012/2024-07-10/2024-07-10/text/original/epub/OEBPS/document_1/document_1.html#_Toc172119199> ;
    dcat:landingPage "https://www.legislation.gov.au/C2020A00012/2024-07-10/2024-07-10/text/original/epub/OEBPS/document_1/document_1.html#_Toc172119199"^^xsd:anyURI ;
    dcat:theme legcons:Division .

C2020A00012:510 a legcons:Division,
        owl:Class,
        dcat:Resource ;
    rdfs:label "Division - D510 Division 3 Obligations and powers of authorised officers"@en-AU ;
    dct:hasPart C2020A00012:511,
        C2020A00012:512 ;
    dct:isPartOf C2020A00012:503 ;
    dct:isReferencedBy C2020A00012: ;
    rdfs:comment "Division 3 Obligations and powers of authorised officers - Abrievated Graph Key: D510"@en-AU ;
    skos:broader C2020A00012:511,
        C2020A00012:512 ;
    skos:definition "Division 3 Obligations and powers of authorised officers"@en-AU ;
    skos:narrower C2020A00012:503 ;
    skos:prefLabel "Division D510"@en-AU ;
    dcat:accessURL <https://www.legislation.gov.au/C2020A00012/2024-07-10/2024-07-10/text/original/epub/OEBPS/document_1/document_1.html#_Toc172119202> ;
    dcat:landingPage "https://www.legislation.gov.au/C2020A00012/2024-07-10/2024-07-10/text/original/epub/OEBPS/document_1/document_1.html#_Toc172119202"^^xsd:anyURI ;
    dcat:theme legcons:Division .

C2020A00012:513 a legcons:Division,
        owl:Class,
        dcat:Resource ;
    rdfs:label "Division - D513 Division 4 Appropriate persons rights and responsibilities"@en-AU ;
    dct:hasPart C2020A00012:514,
        C2020A00012:515 ;
    dct:isPartOf C2020A00012:503 ;
    dct:isReferencedBy C2020A00012: ;
    rdfs:comment "Division 4 Appropriate persons rights and responsibilities - Abrievated Graph Key: D513"@en-AU ;
    skos:broader C2020A00012:514,
        C2020A00012:515 ;
    skos:definition "Division 4 Appropriate persons rights and responsibilities"@en-AU ;
    skos:narrower C2020A00012:503 ;
    skos:prefLabel "Division D513"@en-AU ;
    dcat:accessURL <https://www.legislation.gov.au/C2020A00012/2024-07-10/2024-07-10/text/original/epub/OEBPS/document_1/document_1.html#_Toc172119205> ;
    dcat:landingPage "https://www.legislation.gov.au/C2020A00012/2024-07-10/2024-07-10/text/original/epub/OEBPS/document_1/document_1.html#_Toc172119205"^^xsd:anyURI ;
    dcat:theme legcons:Division .

C2020A00012:516 a legcons:Part,
        owl:Class,
        dcat:Resource ;
    rdfs:label "Part - P516 Part 6 Powers in emergency situations"@en-AU ;
    dct:hasPart C2020A00012:517,
        C2020A00012:519 ;
    dct:isPartOf C2020A00012:467 ;
    dct:isReferencedBy C2020A00012: ;
    rdfs:comment "Part 6 Powers in emergency situations - Abrievated Graph Key: P516"@en-AU ;
    skos:broader C2020A00012:517,
        C2020A00012:519 ;
    skos:definition "Part 6 Powers in emergency situations"@en-AU ;
    skos:narrower C2020A00012:467 ;
    skos:prefLabel "Part P516"@en-AU ;
    dcat:accessURL <https://www.legislation.gov.au/C2020A00012/2024-07-10/2024-07-10/text/original/epub/OEBPS/document_1/document_1.html#_Toc172119208> ;
    dcat:landingPage "https://www.legislation.gov.au/C2020A00012/2024-07-10/2024-07-10/text/original/epub/OEBPS/document_1/document_1.html#_Toc172119208"^^xsd:anyURI ;
    dcat:theme legcons:Part .

C2020A00012:519 a legcons:Division,
        owl:Class,
        dcat:Resource ;
    rdfs:label "Division - D519 Division 2 Powers that may be exercised in or on premises in emergency situations"@en-AU ;
    dct:hasPart C2020A00012:520,
        C2020A00012:521 ;
    dct:isPartOf C2020A00012:516 ;
    dct:isReferencedBy C2020A00012: ;
    rdfs:comment "Division 2 Powers that may be exercised in or on premises in emergency situations - Abrievated Graph Key: D519"@en-AU ;
    skos:broader C2020A00012:520,
        C2020A00012:521 ;
    skos:definition "Division 2 Powers that may be exercised in or on premises in emergency situations"@en-AU ;
    skos:narrower C2020A00012:516 ;
    skos:prefLabel "Division D519"@en-AU ;
    dcat:accessURL <https://www.legislation.gov.au/C2020A00012/2024-07-10/2024-07-10/text/original/epub/OEBPS/document_1/document_1.html#_Toc172119211> ;
    dcat:landingPage "https://www.legislation.gov.au/C2020A00012/2024-07-10/2024-07-10/text/original/epub/OEBPS/document_1/document_1.html#_Toc172119211"^^xsd:anyURI ;
    dcat:theme legcons:Division .

C2020A00012:522 a legcons:Part,
        owl:Class,
        dcat:Resource ;
    rdfs:label "Part - P522 Part 7 Civil penalties"@en-AU ;
    dct:hasPart C2020A00012:523,
        C2020A00012:525 ;
    dct:isPartOf C2020A00012:467 ;
    dct:isReferencedBy C2020A00012: ;
    rdfs:comment "Part 7 Civil penalties - Abrievated Graph Key: P522"@en-AU ;
    skos:broader C2020A00012:523,
        C2020A00012:525 ;
    skos:definition "Part 7 Civil penalties"@en-AU ;
    skos:narrower C2020A00012:467 ;
    skos:prefLabel "Part P522"@en-AU ;
    dcat:accessURL <https://www.legislation.gov.au/C2020A00012/2024-07-10/2024-07-10/text/original/epub/OEBPS/document_1/document_1.html#_Toc172119214> ;
    dcat:landingPage "https://www.legislation.gov.au/C2020A00012/2024-07-10/2024-07-10/text/original/epub/OEBPS/document_1/document_1.html#_Toc172119214"^^xsd:anyURI ;
    dcat:theme legcons:Part .

C2020A00012:527 a legcons:Part,
        owl:Class,
        dcat:Resource ;
    rdfs:label "Part - P527 Part 8 Infringement notices"@en-AU ;
    dct:hasPart C2020A00012:528,
        C2020A00012:530 ;
    dct:isPartOf C2020A00012:467 ;
    dct:isReferencedBy C2020A00012: ;
    rdfs:comment "Part 8 Infringement notices - Abrievated Graph Key: P527"@en-AU ;
    skos:broader C2020A00012:528,
        C2020A00012:530 ;
    skos:definition "Part 8 Infringement notices"@en-AU ;
    skos:narrower C2020A00012:467 ;
    skos:prefLabel "Part P527"@en-AU ;
    dcat:accessURL <https://www.legislation.gov.au/C2020A00012/2024-07-10/2024-07-10/text/original/epub/OEBPS/document_1/document_1.html#_Toc172119219> ;
    dcat:landingPage "https://www.legislation.gov.au/C2020A00012/2024-07-10/2024-07-10/text/original/epub/OEBPS/document_1/document_1.html#_Toc172119219"^^xsd:anyURI ;
    dcat:theme legcons:Part .

C2020A00012:530 a legcons:Division,
        owl:Class,
        dcat:Resource ;
    rdfs:label "Division - D530 Division 2 Infringement notices under Part 5 of the Regulatory Powers Act"@en-AU ;
    dct:hasPart C2020A00012:531,
        C2020A00012:532 ;
    dct:isPartOf C2020A00012:527 ;
    dct:isReferencedBy C2020A00012: ;
    rdfs:comment "Division 2 Infringement notices under Part 5 of the Regulatory Powers Act - Abrievated Graph Key: D530"@en-AU ;
    skos:broader C2020A00012:531,
        C2020A00012:532 ;
    skos:definition "Division 2 Infringement notices under Part 5 of the Regulatory Powers Act"@en-AU ;
    skos:narrower C2020A00012:527 ;
    skos:prefLabel "Division D530"@en-AU ;
    dcat:accessURL <https://www.legislation.gov.au/C2020A00012/2024-07-10/2024-07-10/text/original/epub/OEBPS/document_1/document_1.html#_Toc172119222> ;
    dcat:landingPage "https://www.legislation.gov.au/C2020A00012/2024-07-10/2024-07-10/text/original/epub/OEBPS/document_1/document_1.html#_Toc172119222"^^xsd:anyURI ;
    dcat:theme legcons:Division .

C2020A00012:533 a legcons:Part,
        owl:Class,
        dcat:Resource ;
    rdfs:label "Part - P533 Part 9 Enforceable undertakings"@en-AU ;
    dct:hasPart C2020A00012:534,
        C2020A00012:536 ;
    dct:isPartOf C2020A00012:467 ;
    dct:isReferencedBy C2020A00012: ;
    rdfs:comment "Part 9 Enforceable undertakings - Abrievated Graph Key: P533"@en-AU ;
    skos:broader C2020A00012:534,
        C2020A00012:536 ;
    skos:definition "Part 9 Enforceable undertakings"@en-AU ;
    skos:narrower C2020A00012:467 ;
    skos:prefLabel "Part P533"@en-AU ;
    dcat:accessURL <https://www.legislation.gov.au/C2020A00012/2024-07-10/2024-07-10/text/original/epub/OEBPS/document_1/document_1.html#_Toc172119225> ;
    dcat:landingPage "https://www.legislation.gov.au/C2020A00012/2024-07-10/2024-07-10/text/original/epub/OEBPS/document_1/document_1.html#_Toc172119225"^^xsd:anyURI ;
    dcat:theme legcons:Part .

C2020A00012:538 a legcons:Part,
        owl:Class,
        dcat:Resource ;
    rdfs:label "Part - P538 Part 10 Injunctions"@en-AU ;
    dct:hasPart C2020A00012:539,
        C2020A00012:541 ;
    dct:isPartOf C2020A00012:467 ;
    dct:isReferencedBy C2020A00012: ;
    rdfs:comment "Part 10 Injunctions - Abrievated Graph Key: P538"@en-AU ;
    skos:broader C2020A00012:539,
        C2020A00012:541 ;
    skos:definition "Part 10 Injunctions"@en-AU ;
    skos:narrower C2020A00012:467 ;
    skos:prefLabel "Part P538"@en-AU ;
    dcat:accessURL <https://www.legislation.gov.au/C2020A00012/2024-07-10/2024-07-10/text/original/epub/OEBPS/document_1/document_1.html#_Toc172119230> ;
    dcat:landingPage "https://www.legislation.gov.au/C2020A00012/2024-07-10/2024-07-10/text/original/epub/OEBPS/document_1/document_1.html#_Toc172119230"^^xsd:anyURI ;
    dcat:theme legcons:Part .

C2020A00012:559 a legcons:Division,
        owl:Class,
        dcat:Resource ;
    rdfs:label "Division - D559 Division 4 General rules about offences and civil penalty provisions"@en-AU ;
    dct:hasPart C2020A00012:560,
        C2020A00012:561 ;
    dct:isPartOf C2020A00012:550 ;
    dct:isReferencedBy C2020A00012: ;
    rdfs:comment "Division 4 General rules about offences and civil penalty provisions - Abrievated Graph Key: D559"@en-AU ;
    skos:broader C2020A00012:560,
        C2020A00012:561 ;
    skos:definition "Division 4 General rules about offences and civil penalty provisions"@en-AU ;
    skos:narrower C2020A00012:550 ;
    skos:prefLabel "Division D559"@en-AU ;
    dcat:accessURL <https://www.legislation.gov.au/C2020A00012/2024-07-10/2024-07-10/text/original/epub/OEBPS/document_1/document_1.html#_Toc172119251> ;
    dcat:landingPage "https://www.legislation.gov.au/C2020A00012/2024-07-10/2024-07-10/text/original/epub/OEBPS/document_1/document_1.html#_Toc172119251"^^xsd:anyURI ;
    dcat:theme legcons:Division .

C2020A00012:567 a legcons:Part,
        owl:Class,
        dcat:Resource ;
    rdfs:label "Part - P567 Part 1 Matters relating to applications"@en-AU ;
    dct:hasPart C2020A00012:568,
        C2020A00012:570 ;
    dct:isPartOf C2020A00012:566 ;
    dct:isReferencedBy C2020A00012: ;
    rdfs:comment "Part 1 Matters relating to applications - Abrievated Graph Key: P567"@en-AU ;
    skos:broader C2020A00012:568,
        C2020A00012:570 ;
    skos:definition "Part 1 Matters relating to applications"@en-AU ;
    skos:narrower C2020A00012:566 ;
    skos:prefLabel "Part P567"@en-AU ;
    dcat:accessURL <https://www.legislation.gov.au/C2020A00012/2024-07-10/2024-07-10/text/original/epub/OEBPS/document_1/document_1.html#_Toc172119259> ;
    dcat:landingPage "https://www.legislation.gov.au/C2020A00012/2024-07-10/2024-07-10/text/original/epub/OEBPS/document_1/document_1.html#_Toc172119259"^^xsd:anyURI ;
    dcat:theme legcons:Part .

C2020A00012:575 a legcons:Part,
        owl:Class,
        dcat:Resource ;
    rdfs:label "Part - P575 Part 1 AAlternative regulatory arrangements"@en-AU ;
    dct:hasPart C2020A00012:576,
        C2020A00012:578 ;
    dct:isPartOf C2020A00012:566 ;
    dct:isReferencedBy C2020A00012: ;
    rdfs:comment "Part 1 AAlternative regulatory arrangements - Abrievated Graph Key: P575"@en-AU ;
    skos:broader C2020A00012:576,
        C2020A00012:578 ;
    skos:definition "Part 1 AAlternative regulatory arrangements"@en-AU ;
    skos:narrower C2020A00012:566 ;
    skos:prefLabel "Part P575"@en-AU ;
    dcat:accessURL <https://www.legislation.gov.au/C2020A00012/2024-07-10/2024-07-10/text/original/epub/OEBPS/document_1/document_1.html#_Toc172119267> ;
    dcat:landingPage "https://www.legislation.gov.au/C2020A00012/2024-07-10/2024-07-10/text/original/epub/OEBPS/document_1/document_1.html#_Toc172119267"^^xsd:anyURI ;
    dcat:theme legcons:Part .

C2020A00012:578 a legcons:Division,
        owl:Class,
        dcat:Resource ;
    rdfs:label "Division - D578 Division 2 Alternative regulatory arrangements"@en-AU ;
    dct:hasPart C2020A00012:579,
        C2020A00012:580 ;
    dct:isPartOf C2020A00012:575 ;
    dct:isReferencedBy C2020A00012: ;
    rdfs:comment "Division 2 Alternative regulatory arrangements - Abrievated Graph Key: D578"@en-AU ;
    skos:broader C2020A00012:579,
        C2020A00012:580 ;
    skos:definition "Division 2 Alternative regulatory arrangements"@en-AU ;
    skos:narrower C2020A00012:575 ;
    skos:prefLabel "Division D578"@en-AU ;
    dcat:accessURL <https://www.legislation.gov.au/C2020A00012/2024-07-10/2024-07-10/text/original/epub/OEBPS/document_1/document_1.html#_Toc172119270> ;
    dcat:landingPage "https://www.legislation.gov.au/C2020A00012/2024-07-10/2024-07-10/text/original/epub/OEBPS/document_1/document_1.html#_Toc172119270"^^xsd:anyURI ;
    dcat:theme legcons:Division .

C2020A00012:581 a legcons:Part,
        owl:Class,
        dcat:Resource ;
    rdfs:label "Part - P581 Part 2 Review of decisions"@en-AU ;
    dct:hasPart C2020A00012:582,
        C2020A00012:584 ;
    dct:isPartOf C2020A00012:566 ;
    dct:isReferencedBy C2020A00012: ;
    rdfs:comment "Part 2 Review of decisions - Abrievated Graph Key: P581"@en-AU ;
    skos:broader C2020A00012:582,
        C2020A00012:584 ;
    skos:definition "Part 2 Review of decisions"@en-AU ;
    skos:narrower C2020A00012:566 ;
    skos:prefLabel "Part P581"@en-AU ;
    dcat:accessURL <https://www.legislation.gov.au/C2020A00012/2024-07-10/2024-07-10/text/original/epub/OEBPS/document_1/document_1.html#_Toc172119273> ;
    dcat:landingPage "https://www.legislation.gov.au/C2020A00012/2024-07-10/2024-07-10/text/original/epub/OEBPS/document_1/document_1.html#_Toc172119273"^^xsd:anyURI ;
    dcat:theme legcons:Part .

C2020A00012:610 a legcons:Division,
        owl:Class,
        dcat:Resource ;
    rdfs:label "Division - D610 Division 3 Protected information"@en-AU ;
    dct:hasPart C2020A00012:611,
        C2020A00012:612 ;
    dct:isPartOf C2020A00012:591 ;
    dct:isReferencedBy C2020A00012: ;
    rdfs:comment "Division 3 Protected information - Abrievated Graph Key: D610"@en-AU ;
    skos:broader C2020A00012:611,
        C2020A00012:612 ;
    skos:definition "Division 3 Protected information"@en-AU ;
    skos:narrower C2020A00012:591 ;
    skos:prefLabel "Division D610"@en-AU ;
    dcat:accessURL <https://www.legislation.gov.au/C2020A00012/2024-07-10/2024-07-10/text/original/epub/OEBPS/document_1/document_1.html#_Toc172119302> ;
    dcat:landingPage "https://www.legislation.gov.au/C2020A00012/2024-07-10/2024-07-10/text/original/epub/OEBPS/document_1/document_1.html#_Toc172119302"^^xsd:anyURI ;
    dcat:theme legcons:Division .

C2020A00012:622 a legcons:Division,
        owl:Class,
        dcat:Resource ;
    rdfs:label "Division - D622 Division 4 Unpaid cost recovery charges"@en-AU ;
    dct:hasPart C2020A00012:623,
        C2020A00012:624 ;
    dct:isPartOf C2020A00012:613 ;
    dct:isReferencedBy C2020A00012: ;
    rdfs:comment "Division 4 Unpaid cost recovery charges - Abrievated Graph Key: D622"@en-AU ;
    skos:broader C2020A00012:623,
        C2020A00012:624 ;
    skos:definition "Division 4 Unpaid cost recovery charges"@en-AU ;
    skos:narrower C2020A00012:613 ;
    skos:prefLabel "Division D622"@en-AU ;
    dcat:accessURL <https://www.legislation.gov.au/C2020A00012/2024-07-10/2024-07-10/text/original/epub/OEBPS/document_1/document_1.html#_Toc172119314> ;
    dcat:landingPage "https://www.legislation.gov.au/C2020A00012/2024-07-10/2024-07-10/text/original/epub/OEBPS/document_1/document_1.html#_Toc172119314"^^xsd:anyURI ;
    dcat:theme legcons:Division .

C2020A00012:625 a legcons:Division,
        owl:Class,
        dcat:Resource ;
    rdfs:label "Division - D625 Division 5 Miscellaneous"@en-AU ;
    dct:hasPart C2020A00012:626,
        C2020A00012:627 ;
    dct:isPartOf C2020A00012:613 ;
    dct:isReferencedBy C2020A00012: ;
    rdfs:comment "Division 5 Miscellaneous - Abrievated Graph Key: D625"@en-AU ;
    skos:broader C2020A00012:626,
        C2020A00012:627 ;
    skos:definition "Division 5 Miscellaneous"@en-AU ;
    skos:narrower C2020A00012:613 ;
    skos:prefLabel "Division D625"@en-AU ;
    dcat:accessURL <https://www.legislation.gov.au/C2020A00012/2024-07-10/2024-07-10/text/original/epub/OEBPS/document_1/document_1.html#_Toc172119317> ;
    dcat:landingPage "https://www.legislation.gov.au/C2020A00012/2024-07-10/2024-07-10/text/original/epub/OEBPS/document_1/document_1.html#_Toc172119317"^^xsd:anyURI ;
    dcat:theme legcons:Division .

C2020A00012:628 a legcons:Part,
        owl:Class,
        dcat:Resource ;
    rdfs:label "Part - P628 Part 5 Records"@en-AU ;
    dct:hasPart C2020A00012:629,
        C2020A00012:631 ;
    dct:isPartOf C2020A00012:566 ;
    dct:isReferencedBy C2020A00012: ;
    rdfs:comment "Part 5 Records - Abrievated Graph Key: P628"@en-AU ;
    skos:broader C2020A00012:629,
        C2020A00012:631 ;
    skos:definition "Part 5 Records"@en-AU ;
    skos:narrower C2020A00012:566 ;
    skos:prefLabel "Part P628"@en-AU ;
    dcat:accessURL <https://www.legislation.gov.au/C2020A00012/2024-07-10/2024-07-10/text/original/epub/OEBPS/document_1/document_1.html#_Toc172119320> ;
    dcat:landingPage "https://www.legislation.gov.au/C2020A00012/2024-07-10/2024-07-10/text/original/epub/OEBPS/document_1/document_1.html#_Toc172119320"^^xsd:anyURI ;
    dcat:theme legcons:Part .

C2020A00012:656 a legcons:Division,
        owl:Class,
        dcat:Resource ;
    rdfs:label "Division - D656 Division 6 AAssistance in relation to the phasing out of the export of live sheep by sea"@en-AU ;
    dct:hasPart C2020A00012:657,
        C2020A00012:662 ;
    dct:isPartOf C2020A00012:633 ;
    dct:isReferencedBy C2020A00012: ;
    rdfs:comment "Division 6 AAssistance in relation to the phasing out of the export of live sheep by sea - Abrievated Graph Key: D656"@en-AU ;
    skos:broader C2020A00012:657,
        C2020A00012:662 ;
    skos:definition "Division 6 AAssistance in relation to the phasing out of the export of live sheep by sea"@en-AU ;
    skos:narrower C2020A00012:633 ;
    skos:prefLabel "Division D656"@en-AU ;
    dcat:accessURL <https://www.legislation.gov.au/C2020A00012/2024-07-10/2024-07-10/text/original/epub/OEBPS/document_1/document_1.html#_Toc172119348> ;
    dcat:landingPage "https://www.legislation.gov.au/C2020A00012/2024-07-10/2024-07-10/text/original/epub/OEBPS/document_1/document_1.html#_Toc172119348"^^xsd:anyURI ;
    dcat:theme legcons:Division .

C2020A00012:67 a legcons:Division,
        owl:Class,
        dcat:Resource ;
    rdfs:label "Division - D67 Division 1 Introduction"@en-AU ;
    dct:hasPart C2020A00012:68,
        C2020A00012:69 ;
    dct:isPartOf C2020A00012:27 ;
    dct:isReferencedBy C2020A00012: ;
    rdfs:comment "Division 1 Introduction - Abrievated Graph Key: D67"@en-AU ;
    skos:broader C2020A00012:68,
        C2020A00012:69 ;
    skos:definition "Division 1 Introduction"@en-AU ;
    skos:narrower C2020A00012:27 ;
    skos:prefLabel "Division D67"@en-AU ;
    dcat:accessURL <https://www.legislation.gov.au/C2020A00012/2024-07-10/2024-07-10/text/original/epub/OEBPS/document_1/document_1.html#_Toc172118759> ;
    dcat:landingPage "https://www.legislation.gov.au/C2020A00012/2024-07-10/2024-07-10/text/original/epub/OEBPS/document_1/document_1.html#_Toc172118759"^^xsd:anyURI ;
    dcat:theme legcons:Division .

C2020A00012:115 a legcons:Division,
        owl:Class,
        dcat:Resource ;
    rdfs:label "Division - D115 Division 1 Application by manager"@en-AU ;
    dct:hasPart C2020A00012:116,
        C2020A00012:117,
        C2020A00012:118 ;
    dct:isPartOf C2020A00012:114 ;
    dct:isReferencedBy C2020A00012: ;
    rdfs:comment "Division 1 Application by manager - Abrievated Graph Key: D115"@en-AU ;
    skos:broader C2020A00012:116,
        C2020A00012:117,
        C2020A00012:118 ;
    skos:definition "Division 1 Application by manager"@en-AU ;
    skos:narrower C2020A00012:114 ;
    skos:prefLabel "Division D115"@en-AU ;
    dcat:accessURL <https://www.legislation.gov.au/C2020A00012/2024-07-10/2024-07-10/text/original/epub/OEBPS/document_1/document_1.html#_Toc172118807> ;
    dcat:landingPage "https://www.legislation.gov.au/C2020A00012/2024-07-10/2024-07-10/text/original/epub/OEBPS/document_1/document_1.html#_Toc172118807"^^xsd:anyURI ;
    dcat:theme legcons:Division .

C2020A00012:122 a legcons:Part,
        owl:Class,
        dcat:Resource ;
    rdfs:label "Part - P122 Part 5 Suspension of accreditation"@en-AU ;
    dct:hasPart C2020A00012:123,
        C2020A00012:126,
        C2020A00012:132 ;
    dct:isPartOf C2020A00012:100 ;
    dct:isReferencedBy C2020A00012: ;
    rdfs:comment "Part 5 Suspension of accreditation - Abrievated Graph Key: P122"@en-AU ;
    skos:broader C2020A00012:123,
        C2020A00012:126,
        C2020A00012:132 ;
    skos:definition "Part 5 Suspension of accreditation"@en-AU ;
    skos:narrower C2020A00012:100 ;
    skos:prefLabel "Part P122"@en-AU ;
    dcat:accessURL <https://www.legislation.gov.au/C2020A00012/2024-07-10/2024-07-10/text/original/epub/OEBPS/document_1/document_1.html#_Toc172118814> ;
    dcat:landingPage "https://www.legislation.gov.au/C2020A00012/2024-07-10/2024-07-10/text/original/epub/OEBPS/document_1/document_1.html#_Toc172118814"^^xsd:anyURI ;
    dcat:theme legcons:Part .

C2020A00012:135 a legcons:Part,
        owl:Class,
        dcat:Resource ;
    rdfs:label "Part - P135 Part 6 Revocation of accreditation"@en-AU ;
    dct:hasPart C2020A00012:136,
        C2020A00012:138,
        C2020A00012:142 ;
    dct:isPartOf C2020A00012:100 ;
    dct:isReferencedBy C2020A00012: ;
    rdfs:comment "Part 6 Revocation of accreditation - Abrievated Graph Key: P135"@en-AU ;
    skos:broader C2020A00012:136,
        C2020A00012:138,
        C2020A00012:142 ;
    skos:definition "Part 6 Revocation of accreditation"@en-AU ;
    skos:narrower C2020A00012:100 ;
    skos:prefLabel "Part P135"@en-AU ;
    dcat:accessURL <https://www.legislation.gov.au/C2020A00012/2024-07-10/2024-07-10/text/original/epub/OEBPS/document_1/document_1.html#_Toc172118827> ;
    dcat:landingPage "https://www.legislation.gov.au/C2020A00012/2024-07-10/2024-07-10/text/original/epub/OEBPS/document_1/document_1.html#_Toc172118827"^^xsd:anyURI ;
    dcat:theme legcons:Part .

C2020A00012:138 a legcons:Division,
        owl:Class,
        dcat:Resource ;
    rdfs:label "Division - D138 Division 2 Revocation by Secretary"@en-AU ;
    dct:hasPart C2020A00012:139,
        C2020A00012:140,
        C2020A00012:141 ;
    dct:isPartOf C2020A00012:135 ;
    dct:isReferencedBy C2020A00012: ;
    rdfs:comment "Division 2 Revocation by Secretary - Abrievated Graph Key: D138"@en-AU ;
    skos:broader C2020A00012:139,
        C2020A00012:140,
        C2020A00012:141 ;
    skos:definition "Division 2 Revocation by Secretary"@en-AU ;
    skos:narrower C2020A00012:135 ;
    skos:prefLabel "Division D138"@en-AU ;
    dcat:accessURL <https://www.legislation.gov.au/C2020A00012/2024-07-10/2024-07-10/text/original/epub/OEBPS/document_1/document_1.html#_Toc172118830> ;
    dcat:landingPage "https://www.legislation.gov.au/C2020A00012/2024-07-10/2024-07-10/text/original/epub/OEBPS/document_1/document_1.html#_Toc172118830"^^xsd:anyURI ;
    dcat:theme legcons:Division .

C2020A00012:164 a legcons:Division,
        owl:Class,
        dcat:Resource ;
    rdfs:label "Division - D164 Division 1 Application by occupier"@en-AU ;
    dct:hasPart C2020A00012:165,
        C2020A00012:166,
        C2020A00012:167 ;
    dct:isPartOf C2020A00012:163 ;
    dct:isReferencedBy C2020A00012: ;
    rdfs:comment "Division 1 Application by occupier - Abrievated Graph Key: D164"@en-AU ;
    skos:broader C2020A00012:165,
        C2020A00012:166,
        C2020A00012:167 ;
    skos:definition "Division 1 Application by occupier"@en-AU ;
    skos:narrower C2020A00012:163 ;
    skos:prefLabel "Division D164"@en-AU ;
    dcat:accessURL <https://www.legislation.gov.au/C2020A00012/2024-07-10/2024-07-10/text/original/epub/OEBPS/document_1/document_1.html#_Toc172118856> ;
    dcat:landingPage "https://www.legislation.gov.au/C2020A00012/2024-07-10/2024-07-10/text/original/epub/OEBPS/document_1/document_1.html#_Toc172118856"^^xsd:anyURI ;
    dcat:theme legcons:Division .

C2020A00012:181 a legcons:Division,
        owl:Class,
        dcat:Resource ;
    rdfs:label "Division - D181 Division 3 Direction to cease carrying out export operations"@en-AU ;
    dct:hasPart C2020A00012:182,
        C2020A00012:183,
        C2020A00012:184 ;
    dct:isPartOf C2020A00012:171 ;
    dct:isReferencedBy C2020A00012: ;
    rdfs:comment "Division 3 Direction to cease carrying out export operations - Abrievated Graph Key: D181"@en-AU ;
    skos:broader C2020A00012:182,
        C2020A00012:183,
        C2020A00012:184 ;
    skos:definition "Division 3 Direction to cease carrying out export operations"@en-AU ;
    skos:narrower C2020A00012:171 ;
    skos:prefLabel "Division D181"@en-AU ;
    dcat:accessURL <https://www.legislation.gov.au/C2020A00012/2024-07-10/2024-07-10/text/original/epub/OEBPS/document_1/document_1.html#_Toc172118873> ;
    dcat:landingPage "https://www.legislation.gov.au/C2020A00012/2024-07-10/2024-07-10/text/original/epub/OEBPS/document_1/document_1.html#_Toc172118873"^^xsd:anyURI ;
    dcat:theme legcons:Division .

C2020A00012:188 a legcons:Part,
        owl:Class,
        dcat:Resource ;
    rdfs:label "Part - P188 Part 6 Revocation of registration"@en-AU ;
    dct:hasPart C2020A00012:189,
        C2020A00012:191,
        C2020A00012:195 ;
    dct:isPartOf C2020A00012:149 ;
    dct:isReferencedBy C2020A00012: ;
    rdfs:comment "Part 6 Revocation of registration - Abrievated Graph Key: P188"@en-AU ;
    skos:broader C2020A00012:189,
        C2020A00012:191,
        C2020A00012:195 ;
    skos:definition "Part 6 Revocation of registration"@en-AU ;
    skos:narrower C2020A00012:149 ;
    skos:prefLabel "Part P188"@en-AU ;
    dcat:accessURL <https://www.legislation.gov.au/C2020A00012/2024-07-10/2024-07-10/text/original/epub/OEBPS/document_1/document_1.html#_Toc172118880> ;
    dcat:landingPage "https://www.legislation.gov.au/C2020A00012/2024-07-10/2024-07-10/text/original/epub/OEBPS/document_1/document_1.html#_Toc172118880"^^xsd:anyURI ;
    dcat:theme legcons:Part .

C2020A00012:191 a legcons:Division,
        owl:Class,
        dcat:Resource ;
    rdfs:label "Division - D191 Division 2 Revocation by Secretary"@en-AU ;
    dct:hasPart C2020A00012:192,
        C2020A00012:193,
        C2020A00012:194 ;
    dct:isPartOf C2020A00012:188 ;
    dct:isReferencedBy C2020A00012: ;
    rdfs:comment "Division 2 Revocation by Secretary - Abrievated Graph Key: D191"@en-AU ;
    skos:broader C2020A00012:192,
        C2020A00012:193,
        C2020A00012:194 ;
    skos:definition "Division 2 Revocation by Secretary"@en-AU ;
    skos:narrower C2020A00012:188 ;
    skos:prefLabel "Division D191"@en-AU ;
    dcat:accessURL <https://www.legislation.gov.au/C2020A00012/2024-07-10/2024-07-10/text/original/epub/OEBPS/document_1/document_1.html#_Toc172118883> ;
    dcat:landingPage "https://www.legislation.gov.au/C2020A00012/2024-07-10/2024-07-10/text/original/epub/OEBPS/document_1/document_1.html#_Toc172118883"^^xsd:anyURI ;
    dcat:theme legcons:Division .

C2020A00012:221 a legcons:Division,
        owl:Class,
        dcat:Resource ;
    rdfs:label "Division - D221 Division 1 Variations by holder"@en-AU ;
    dct:hasPart C2020A00012:222,
        C2020A00012:225,
        C2020A00012:229 ;
    dct:isPartOf C2020A00012:220 ;
    dct:isReferencedBy C2020A00012: ;
    rdfs:comment "Division 1 Variations by holder - Abrievated Graph Key: D221"@en-AU ;
    skos:broader C2020A00012:222,
        C2020A00012:225,
        C2020A00012:229 ;
    skos:definition "Division 1 Variations by holder"@en-AU ;
    skos:narrower C2020A00012:220 ;
    skos:prefLabel "Division D221"@en-AU ;
    dcat:accessURL <https://www.legislation.gov.au/C2020A00012/2024-07-10/2024-07-10/text/original/epub/OEBPS/document_1/document_1.html#_Toc172118913> ;
    dcat:landingPage "https://www.legislation.gov.au/C2020A00012/2024-07-10/2024-07-10/text/original/epub/OEBPS/document_1/document_1.html#_Toc172118913"^^xsd:anyURI ;
    dcat:theme legcons:Division .

C2020A00012:225 a legcons:Subdivision,
        owl:Class,
        dcat:Resource ;
    rdfs:label "Subdivision - S225 Subdivision BSignificant variations and variation of conditions"@en-AU ;
    dct:hasPart C2020A00012:226,
        C2020A00012:227,
        C2020A00012:228 ;
    dct:isPartOf C2020A00012:221 ;
    dct:isReferencedBy C2020A00012: ;
    rdfs:comment "Subdivision BSignificant variations and variation of conditions - Abrievated Graph Key: S225"@en-AU ;
    skos:broader C2020A00012:226,
        C2020A00012:227,
        C2020A00012:228 ;
    skos:definition "Subdivision BSignificant variations and variation of conditions"@en-AU ;
    skos:narrower C2020A00012:221 ;
    skos:prefLabel "Subdivision S225"@en-AU ;
    dcat:accessURL <https://www.legislation.gov.au/C2020A00012/2024-07-10/2024-07-10/text/original/epub/OEBPS/document_1/document_1.html#_Toc172118917> ;
    dcat:landingPage "https://www.legislation.gov.au/C2020A00012/2024-07-10/2024-07-10/text/original/epub/OEBPS/document_1/document_1.html#_Toc172118917"^^xsd:anyURI ;
    dcat:theme legcons:Subdivision .

C2020A00012:236 a legcons:Part,
        owl:Class,
        dcat:Resource ;
    rdfs:label "Part - P236 Part 5 Suspension of approved arrangement"@en-AU ;
    dct:hasPart C2020A00012:237,
        C2020A00012:240,
        C2020A00012:246 ;
    dct:isPartOf C2020A00012:206 ;
    dct:isReferencedBy C2020A00012: ;
    rdfs:comment "Part 5 Suspension of approved arrangement - Abrievated Graph Key: P236"@en-AU ;
    skos:broader C2020A00012:237,
        C2020A00012:240,
        C2020A00012:246 ;
    skos:definition "Part 5 Suspension of approved arrangement"@en-AU ;
    skos:narrower C2020A00012:206 ;
    skos:prefLabel "Part P236"@en-AU ;
    dcat:accessURL <https://www.legislation.gov.au/C2020A00012/2024-07-10/2024-07-10/text/original/epub/OEBPS/document_1/document_1.html#_Toc172118928> ;
    dcat:landingPage "https://www.legislation.gov.au/C2020A00012/2024-07-10/2024-07-10/text/original/epub/OEBPS/document_1/document_1.html#_Toc172118928"^^xsd:anyURI ;
    dcat:theme legcons:Part .

C2020A00012:249 a legcons:Part,
        owl:Class,
        dcat:Resource ;
    rdfs:label "Part - P249 Part 6 Revocation of approved arrangement"@en-AU ;
    dct:hasPart C2020A00012:250,
        C2020A00012:252,
        C2020A00012:256 ;
    dct:isPartOf C2020A00012:206 ;
    dct:isReferencedBy C2020A00012: ;
    rdfs:comment "Part 6 Revocation of approved arrangement - Abrievated Graph Key: P249"@en-AU ;
    skos:broader C2020A00012:250,
        C2020A00012:252,
        C2020A00012:256 ;
    skos:definition "Part 6 Revocation of approved arrangement"@en-AU ;
    skos:narrower C2020A00012:206 ;
    skos:prefLabel "Part P249"@en-AU ;
    dcat:accessURL <https://www.legislation.gov.au/C2020A00012/2024-07-10/2024-07-10/text/original/epub/OEBPS/document_1/document_1.html#_Toc172118941> ;
    dcat:landingPage "https://www.legislation.gov.au/C2020A00012/2024-07-10/2024-07-10/text/original/epub/OEBPS/document_1/document_1.html#_Toc172118941"^^xsd:anyURI ;
    dcat:theme legcons:Part .

C2020A00012:252 a legcons:Division,
        owl:Class,
        dcat:Resource ;
    rdfs:label "Division - D252 Division 2 Revocation by Secretary"@en-AU ;
    dct:hasPart C2020A00012:253,
        C2020A00012:254,
        C2020A00012:255 ;
    dct:isPartOf C2020A00012:249 ;
    dct:isReferencedBy C2020A00012: ;
    rdfs:comment "Division 2 Revocation by Secretary - Abrievated Graph Key: D252"@en-AU ;
    skos:broader C2020A00012:253,
        C2020A00012:254,
        C2020A00012:255 ;
    skos:definition "Division 2 Revocation by Secretary"@en-AU ;
    skos:narrower C2020A00012:249 ;
    skos:prefLabel "Division D252"@en-AU ;
    dcat:accessURL <https://www.legislation.gov.au/C2020A00012/2024-07-10/2024-07-10/text/original/epub/OEBPS/document_1/document_1.html#_Toc172118944> ;
    dcat:landingPage "https://www.legislation.gov.au/C2020A00012/2024-07-10/2024-07-10/text/original/epub/OEBPS/document_1/document_1.html#_Toc172118944"^^xsd:anyURI ;
    dcat:theme legcons:Division .

C2020A00012:286 a legcons:Part,
        owl:Class,
        dcat:Resource ;
    rdfs:label "Part - P286 Part 5 Suspension of export licence"@en-AU ;
    dct:hasPart C2020A00012:287,
        C2020A00012:290,
        C2020A00012:296 ;
    dct:isPartOf C2020A00012:265 ;
    dct:isReferencedBy C2020A00012: ;
    rdfs:comment "Part 5 Suspension of export licence - Abrievated Graph Key: P286"@en-AU ;
    skos:broader C2020A00012:287,
        C2020A00012:290,
        C2020A00012:296 ;
    skos:definition "Part 5 Suspension of export licence"@en-AU ;
    skos:narrower C2020A00012:265 ;
    skos:prefLabel "Part P286"@en-AU ;
    dcat:accessURL <https://www.legislation.gov.au/C2020A00012/2024-07-10/2024-07-10/text/original/epub/OEBPS/document_1/document_1.html#_Toc172118978> ;
    dcat:landingPage "https://www.legislation.gov.au/C2020A00012/2024-07-10/2024-07-10/text/original/epub/OEBPS/document_1/document_1.html#_Toc172118978"^^xsd:anyURI ;
    dcat:theme legcons:Part .

C2020A00012:298 a legcons:Part,
        owl:Class,
        dcat:Resource ;
    rdfs:label "Part - P298 Part 6 Revocation of export licence"@en-AU ;
    dct:hasPart C2020A00012:299,
        C2020A00012:301,
        C2020A00012:305 ;
    dct:isPartOf C2020A00012:265 ;
    dct:isReferencedBy C2020A00012: ;
    rdfs:comment "Part 6 Revocation of export licence - Abrievated Graph Key: P298"@en-AU ;
    skos:broader C2020A00012:299,
        C2020A00012:301,
        C2020A00012:305 ;
    skos:definition "Part 6 Revocation of export licence"@en-AU ;
    skos:narrower C2020A00012:265 ;
    skos:prefLabel "Part P298"@en-AU ;
    dcat:accessURL <https://www.legislation.gov.au/C2020A00012/2024-07-10/2024-07-10/text/original/epub/OEBPS/document_1/document_1.html#_Toc172118990> ;
    dcat:landingPage "https://www.legislation.gov.au/C2020A00012/2024-07-10/2024-07-10/text/original/epub/OEBPS/document_1/document_1.html#_Toc172118990"^^xsd:anyURI ;
    dcat:theme legcons:Part .

C2020A00012:301 a legcons:Division,
        owl:Class,
        dcat:Resource ;
    rdfs:label "Division - D301 Division 2 Revocation by Secretary"@en-AU ;
    dct:hasPart C2020A00012:302,
        C2020A00012:303,
        C2020A00012:304 ;
    dct:isPartOf C2020A00012:298 ;
    dct:isReferencedBy C2020A00012: ;
    rdfs:comment "Division 2 Revocation by Secretary - Abrievated Graph Key: D301"@en-AU ;
    skos:broader C2020A00012:302,
        C2020A00012:303,
        C2020A00012:304 ;
    skos:definition "Division 2 Revocation by Secretary"@en-AU ;
    skos:narrower C2020A00012:298 ;
    skos:prefLabel "Division D301"@en-AU ;
    dcat:accessURL <https://www.legislation.gov.au/C2020A00012/2024-07-10/2024-07-10/text/original/epub/OEBPS/document_1/document_1.html#_Toc172118993> ;
    dcat:landingPage "https://www.legislation.gov.au/C2020A00012/2024-07-10/2024-07-10/text/original/epub/OEBPS/document_1/document_1.html#_Toc172118993"^^xsd:anyURI ;
    dcat:theme legcons:Division .

C2020A00012:308 a legcons:Part,
        owl:Class,
        dcat:Resource ;
    rdfs:label "Part - P308 Part 7 Obligations of holders of export licences"@en-AU ;
    dct:hasPart C2020A00012:309,
        C2020A00012:310,
        C2020A00012:311 ;
    dct:isPartOf C2020A00012:265 ;
    dct:isReferencedBy C2020A00012: ;
    rdfs:comment "Part 7 Obligations of holders of export licences - Abrievated Graph Key: P308"@en-AU ;
    skos:broader C2020A00012:309,
        C2020A00012:310,
        C2020A00012:311 ;
    skos:definition "Part 7 Obligations of holders of export licences"@en-AU ;
    skos:narrower C2020A00012:265 ;
    skos:prefLabel "Part P308"@en-AU ;
    dcat:accessURL <https://www.legislation.gov.au/C2020A00012/2024-07-10/2024-07-10/text/original/epub/OEBPS/document_1/document_1.html#_Toc172119000> ;
    dcat:landingPage "https://www.legislation.gov.au/C2020A00012/2024-07-10/2024-07-10/text/original/epub/OEBPS/document_1/document_1.html#_Toc172119000"^^xsd:anyURI ;
    dcat:theme legcons:Part .

C2020A00012:312 a legcons:Part,
        owl:Class,
        dcat:Resource ;
    rdfs:label "Part - P312 Part 8 Other matters"@en-AU ;
    dct:hasPart C2020A00012:313,
        C2020A00012:314,
        C2020A00012:315 ;
    dct:isPartOf C2020A00012:265 ;
    dct:isReferencedBy C2020A00012: ;
    rdfs:comment "Part 8 Other matters - Abrievated Graph Key: P312"@en-AU ;
    skos:broader C2020A00012:313,
        C2020A00012:314,
        C2020A00012:315 ;
    skos:definition "Part 8 Other matters"@en-AU ;
    skos:narrower C2020A00012:265 ;
    skos:prefLabel "Part P312"@en-AU ;
    dcat:accessURL <https://www.legislation.gov.au/C2020A00012/2024-07-10/2024-07-10/text/original/epub/OEBPS/document_1/document_1.html#_Toc172119004> ;
    dcat:landingPage "https://www.legislation.gov.au/C2020A00012/2024-07-10/2024-07-10/text/original/epub/OEBPS/document_1/document_1.html#_Toc172119004"^^xsd:anyURI ;
    dcat:theme legcons:Part .

C2020A00012:341 a legcons:Chapter,
        owl:Class,
        dcat:Resource ;
    rdfs:label "Chapter - C341 Chapter 8 Other matters relating to export"@en-AU ;
    dct:hasPart C2020A00012:342,
        C2020A00012:348,
        C2020A00012:361,
        C2020A00012:374 ;
    dct:isReferencedBy C2020A00012: ;
    rdfs:comment "Chapter 8 Other matters relating to export - Abrievated Graph Key: C341"@en-AU ;
    skos:broader C2020A00012:342,
        C2020A00012:348,
        C2020A00012:361,
        C2020A00012:374 ;
    skos:definition "Chapter 8 Other matters relating to export"@en-AU ;
    skos:prefLabel "Chapter C341"@en-AU ;
    dcat:accessURL <https://www.legislation.gov.au/C2020A00012/2024-07-10/2024-07-10/text/original/epub/OEBPS/document_1/document_1.html#_Toc172119033> ;
    dcat:landingPage "https://www.legislation.gov.au/C2020A00012/2024-07-10/2024-07-10/text/original/epub/OEBPS/document_1/document_1.html#_Toc172119033"^^xsd:anyURI ;
    dcat:theme legcons:Chapter .

C2020A00012:348 a legcons:Part,
        owl:Class,
        dcat:Resource ;
    rdfs:label "Part - P348 Part 2 Trade descriptions"@en-AU ;
    dct:hasPart C2020A00012:349,
        C2020A00012:351,
        C2020A00012:357 ;
    dct:isPartOf C2020A00012:341 ;
    dct:isReferencedBy C2020A00012: ;
    rdfs:comment "Part 2 Trade descriptions - Abrievated Graph Key: P348"@en-AU ;
    skos:broader C2020A00012:349,
        C2020A00012:351,
        C2020A00012:357 ;
    skos:definition "Part 2 Trade descriptions"@en-AU ;
    skos:narrower C2020A00012:341 ;
    skos:prefLabel "Part P348"@en-AU ;
    dcat:accessURL <https://www.legislation.gov.au/C2020A00012/2024-07-10/2024-07-10/text/original/epub/OEBPS/document_1/document_1.html#_Toc172119040> ;
    dcat:landingPage "https://www.legislation.gov.au/C2020A00012/2024-07-10/2024-07-10/text/original/epub/OEBPS/document_1/document_1.html#_Toc172119040"^^xsd:anyURI ;
    dcat:theme legcons:Part .

C2020A00012:357 a legcons:Division,
        owl:Class,
        dcat:Resource ;
    rdfs:label "Division - D357 Division 3 False trade descriptions for prescribed goods"@en-AU ;
    dct:hasPart C2020A00012:358,
        C2020A00012:359,
        C2020A00012:360 ;
    dct:isPartOf C2020A00012:348 ;
    dct:isReferencedBy C2020A00012: ;
    rdfs:comment "Division 3 False trade descriptions for prescribed goods - Abrievated Graph Key: D357"@en-AU ;
    skos:broader C2020A00012:358,
        C2020A00012:359,
        C2020A00012:360 ;
    skos:definition "Division 3 False trade descriptions for prescribed goods"@en-AU ;
    skos:narrower C2020A00012:348 ;
    skos:prefLabel "Division D357"@en-AU ;
    dcat:accessURL <https://www.legislation.gov.au/C2020A00012/2024-07-10/2024-07-10/text/original/epub/OEBPS/document_1/document_1.html#_Toc172119049> ;
    dcat:landingPage "https://www.legislation.gov.au/C2020A00012/2024-07-10/2024-07-10/text/original/epub/OEBPS/document_1/document_1.html#_Toc172119049"^^xsd:anyURI ;
    dcat:theme legcons:Division .

C2020A00012:361 a legcons:Part,
        owl:Class,
        dcat:Resource ;
    rdfs:label "Part - P361 Part 3 Official marks"@en-AU ;
    dct:hasPart C2020A00012:362,
        C2020A00012:364,
        C2020A00012:368 ;
    dct:isPartOf C2020A00012:341 ;
    dct:isReferencedBy C2020A00012: ;
    rdfs:comment "Part 3 Official marks - Abrievated Graph Key: P361"@en-AU ;
    skos:broader C2020A00012:362,
        C2020A00012:364,
        C2020A00012:368 ;
    skos:definition "Part 3 Official marks"@en-AU ;
    skos:narrower C2020A00012:341 ;
    skos:prefLabel "Part P361"@en-AU ;
    dcat:accessURL <https://www.legislation.gov.au/C2020A00012/2024-07-10/2024-07-10/text/original/epub/OEBPS/document_1/document_1.html#_Toc172119053> ;
    dcat:landingPage "https://www.legislation.gov.au/C2020A00012/2024-07-10/2024-07-10/text/original/epub/OEBPS/document_1/document_1.html#_Toc172119053"^^xsd:anyURI ;
    dcat:theme legcons:Part .

C2020A00012:364 a legcons:Division,
        owl:Class,
        dcat:Resource ;
    rdfs:label "Division - D364 Division 2 Rule making powers"@en-AU ;
    dct:hasPart C2020A00012:365,
        C2020A00012:366,
        C2020A00012:367 ;
    dct:isPartOf C2020A00012:361 ;
    dct:isReferencedBy C2020A00012: ;
    rdfs:comment "Division 2 Rule making powers - Abrievated Graph Key: D364"@en-AU ;
    skos:broader C2020A00012:365,
        C2020A00012:366,
        C2020A00012:367 ;
    skos:definition "Division 2 Rule making powers"@en-AU ;
    skos:narrower C2020A00012:361 ;
    skos:prefLabel "Division D364"@en-AU ;
    dcat:accessURL <https://www.legislation.gov.au/C2020A00012/2024-07-10/2024-07-10/text/original/epub/OEBPS/document_1/document_1.html#_Toc172119056> ;
    dcat:landingPage "https://www.legislation.gov.au/C2020A00012/2024-07-10/2024-07-10/text/original/epub/OEBPS/document_1/document_1.html#_Toc172119056"^^xsd:anyURI ;
    dcat:theme legcons:Division .

C2020A00012:380 a legcons:Part,
        owl:Class,
        dcat:Resource ;
    rdfs:label "Part - P380 Part 1 Audits"@en-AU ;
    dct:hasPart C2020A00012:381,
        C2020A00012:383,
        C2020A00012:391 ;
    dct:isPartOf C2020A00012:379 ;
    dct:isReferencedBy C2020A00012: ;
    rdfs:comment "Part 1 Audits - Abrievated Graph Key: P380"@en-AU ;
    skos:broader C2020A00012:381,
        C2020A00012:383,
        C2020A00012:391 ;
    skos:definition "Part 1 Audits"@en-AU ;
    skos:narrower C2020A00012:379 ;
    skos:prefLabel "Part P380"@en-AU ;
    dcat:accessURL <https://www.legislation.gov.au/C2020A00012/2024-07-10/2024-07-10/text/original/epub/OEBPS/document_1/document_1.html#_Toc172119072> ;
    dcat:landingPage "https://www.legislation.gov.au/C2020A00012/2024-07-10/2024-07-10/text/original/epub/OEBPS/document_1/document_1.html#_Toc172119072"^^xsd:anyURI ;
    dcat:theme legcons:Part .

C2020A00012:391 a legcons:Division,
        owl:Class,
        dcat:Resource ;
    rdfs:label "Division - D391 Division 3 Approved auditors"@en-AU ;
    dct:hasPart C2020A00012:392,
        C2020A00012:393,
        C2020A00012:394 ;
    dct:isPartOf C2020A00012:380 ;
    dct:isReferencedBy C2020A00012: ;
    rdfs:comment "Division 3 Approved auditors - Abrievated Graph Key: D391"@en-AU ;
    skos:broader C2020A00012:392,
        C2020A00012:393,
        C2020A00012:394 ;
    skos:definition "Division 3 Approved auditors"@en-AU ;
    skos:narrower C2020A00012:380 ;
    skos:prefLabel "Division D391"@en-AU ;
    dcat:accessURL <https://www.legislation.gov.au/C2020A00012/2024-07-10/2024-07-10/text/original/epub/OEBPS/document_1/document_1.html#_Toc172119083> ;
    dcat:landingPage "https://www.legislation.gov.au/C2020A00012/2024-07-10/2024-07-10/text/original/epub/OEBPS/document_1/document_1.html#_Toc172119083"^^xsd:anyURI ;
    dcat:theme legcons:Division .

C2020A00012:395 a legcons:Part,
        owl:Class,
        dcat:Resource ;
    rdfs:label "Part - P395 Part 2 Assessment of goods"@en-AU ;
    dct:hasPart C2020A00012:396,
        C2020A00012:398,
        C2020A00012:403 ;
    dct:isPartOf C2020A00012:379 ;
    dct:isReferencedBy C2020A00012: ;
    rdfs:comment "Part 2 Assessment of goods - Abrievated Graph Key: P395"@en-AU ;
    skos:broader C2020A00012:396,
        C2020A00012:398,
        C2020A00012:403 ;
    skos:definition "Part 2 Assessment of goods"@en-AU ;
    skos:narrower C2020A00012:379 ;
    skos:prefLabel "Part P395"@en-AU ;
    dcat:accessURL <https://www.legislation.gov.au/C2020A00012/2024-07-10/2024-07-10/text/original/epub/OEBPS/document_1/document_1.html#_Toc172119087> ;
    dcat:landingPage "https://www.legislation.gov.au/C2020A00012/2024-07-10/2024-07-10/text/original/epub/OEBPS/document_1/document_1.html#_Toc172119087"^^xsd:anyURI ;
    dcat:theme legcons:Part .

C2020A00012:403 a legcons:Division,
        owl:Class,
        dcat:Resource ;
    rdfs:label "Division - D403 Division 3 Approved assessors"@en-AU ;
    dct:hasPart C2020A00012:404,
        C2020A00012:405,
        C2020A00012:406 ;
    dct:isPartOf C2020A00012:395 ;
    dct:isReferencedBy C2020A00012: ;
    rdfs:comment "Division 3 Approved assessors - Abrievated Graph Key: D403"@en-AU ;
    skos:broader C2020A00012:404,
        C2020A00012:405,
        C2020A00012:406 ;
    skos:definition "Division 3 Approved assessors"@en-AU ;
    skos:narrower C2020A00012:395 ;
    skos:prefLabel "Division D403"@en-AU ;
    dcat:accessURL <https://www.legislation.gov.au/C2020A00012/2024-07-10/2024-07-10/text/original/epub/OEBPS/document_1/document_1.html#_Toc172119095> ;
    dcat:landingPage "https://www.legislation.gov.au/C2020A00012/2024-07-10/2024-07-10/text/original/epub/OEBPS/document_1/document_1.html#_Toc172119095"^^xsd:anyURI ;
    dcat:theme legcons:Division .

C2020A00012:424 a legcons:Division,
        owl:Class,
        dcat:Resource ;
    rdfs:label "Division - D424 Division 3 Variation suspension and revocation of authorisation"@en-AU ;
    dct:hasPart C2020A00012:425,
        C2020A00012:430,
        C2020A00012:435 ;
    dct:isPartOf C2020A00012:416 ;
    dct:isReferencedBy C2020A00012: ;
    rdfs:comment "Division 3 Variation suspension and revocation of authorisation - Abrievated Graph Key: D424"@en-AU ;
    skos:broader C2020A00012:425,
        C2020A00012:430,
        C2020A00012:435 ;
    skos:definition "Division 3 Variation suspension and revocation of authorisation"@en-AU ;
    skos:narrower C2020A00012:416 ;
    skos:prefLabel "Division D424"@en-AU ;
    dcat:accessURL <https://www.legislation.gov.au/C2020A00012/2024-07-10/2024-07-10/text/original/epub/OEBPS/document_1/document_1.html#_Toc172119116> ;
    dcat:landingPage "https://www.legislation.gov.au/C2020A00012/2024-07-10/2024-07-10/text/original/epub/OEBPS/document_1/document_1.html#_Toc172119116"^^xsd:anyURI ;
    dcat:theme legcons:Division .

C2020A00012:555 a legcons:Division,
        owl:Class,
        dcat:Resource ;
    rdfs:label "Division - D555 Division 3 Civil penalty provisions for false or misleading information or documents"@en-AU ;
    dct:hasPart C2020A00012:556,
        C2020A00012:557,
        C2020A00012:558 ;
    dct:isPartOf C2020A00012:550 ;
    dct:isReferencedBy C2020A00012: ;
    rdfs:comment "Division 3 Civil penalty provisions for false or misleading information or documents - Abrievated Graph Key: D555"@en-AU ;
    skos:broader C2020A00012:556,
        C2020A00012:557,
        C2020A00012:558 ;
    skos:definition "Division 3 Civil penalty provisions for false or misleading information or documents"@en-AU ;
    skos:narrower C2020A00012:550 ;
    skos:prefLabel "Division D555"@en-AU ;
    dcat:accessURL <https://www.legislation.gov.au/C2020A00012/2024-07-10/2024-07-10/text/original/epub/OEBPS/document_1/document_1.html#_Toc172119247> ;
    dcat:landingPage "https://www.legislation.gov.au/C2020A00012/2024-07-10/2024-07-10/text/original/epub/OEBPS/document_1/document_1.html#_Toc172119247"^^xsd:anyURI ;
    dcat:theme legcons:Division .

C2020A00012:562 a legcons:Division,
        owl:Class,
        dcat:Resource ;
    rdfs:label "Division - D562 Division 5 Fit and proper person test"@en-AU ;
    dct:hasPart C2020A00012:563,
        C2020A00012:564,
        C2020A00012:565 ;
    dct:isPartOf C2020A00012:550 ;
    dct:isReferencedBy C2020A00012: ;
    rdfs:comment "Division 5 Fit and proper person test - Abrievated Graph Key: D562"@en-AU ;
    skos:broader C2020A00012:563,
        C2020A00012:564,
        C2020A00012:565 ;
    skos:definition "Division 5 Fit and proper person test"@en-AU ;
    skos:narrower C2020A00012:550 ;
    skos:prefLabel "Division D562"@en-AU ;
    dcat:accessURL <https://www.legislation.gov.au/C2020A00012/2024-07-10/2024-07-10/text/original/epub/OEBPS/document_1/document_1.html#_Toc172119254> ;
    dcat:landingPage "https://www.legislation.gov.au/C2020A00012/2024-07-10/2024-07-10/text/original/epub/OEBPS/document_1/document_1.html#_Toc172119254"^^xsd:anyURI ;
    dcat:theme legcons:Division .

C2020A00012:591 a legcons:Part,
        owl:Class,
        dcat:Resource ;
    rdfs:label "Part - P591 Part 3 Information management"@en-AU ;
    dct:hasPart C2020A00012:592,
        C2020A00012:594,
        C2020A00012:610 ;
    dct:isPartOf C2020A00012:566 ;
    dct:isReferencedBy C2020A00012: ;
    rdfs:comment "Part 3 Information management - Abrievated Graph Key: P591"@en-AU ;
    skos:broader C2020A00012:592,
        C2020A00012:594,
        C2020A00012:610 ;
    skos:definition "Part 3 Information management"@en-AU ;
    skos:narrower C2020A00012:566 ;
    skos:prefLabel "Part P591"@en-AU ;
    dcat:accessURL <https://www.legislation.gov.au/C2020A00012/2024-07-10/2024-07-10/text/original/epub/OEBPS/document_1/document_1.html#_Toc172119283> ;
    dcat:landingPage "https://www.legislation.gov.au/C2020A00012/2024-07-10/2024-07-10/text/original/epub/OEBPS/document_1/document_1.html#_Toc172119283"^^xsd:anyURI ;
    dcat:theme legcons:Part .

C2020A00012:618 a legcons:Division,
        owl:Class,
        dcat:Resource ;
    rdfs:label "Division - D618 Division 3 Payment of cost recovery charges"@en-AU ;
    dct:hasPart C2020A00012:619,
        C2020A00012:620,
        C2020A00012:621 ;
    dct:isPartOf C2020A00012:613 ;
    dct:isReferencedBy C2020A00012: ;
    rdfs:comment "Division 3 Payment of cost recovery charges - Abrievated Graph Key: D618"@en-AU ;
    skos:broader C2020A00012:619,
        C2020A00012:620,
        C2020A00012:621 ;
    skos:definition "Division 3 Payment of cost recovery charges"@en-AU ;
    skos:narrower C2020A00012:613 ;
    skos:prefLabel "Division D618"@en-AU ;
    dcat:accessURL <https://www.legislation.gov.au/C2020A00012/2024-07-10/2024-07-10/text/original/epub/OEBPS/document_1/document_1.html#_Toc172119310> ;
    dcat:landingPage "https://www.legislation.gov.au/C2020A00012/2024-07-10/2024-07-10/text/original/epub/OEBPS/document_1/document_1.html#_Toc172119310"^^xsd:anyURI ;
    dcat:theme legcons:Division .

C2020A00012:650 a legcons:Division,
        owl:Class,
        dcat:Resource ;
    rdfs:label "Division - D650 Division 5 Partnerships unincorporated associations and trusts"@en-AU ;
    dct:hasPart C2020A00012:651,
        C2020A00012:652,
        C2020A00012:653 ;
    dct:isPartOf C2020A00012:633 ;
    dct:isReferencedBy C2020A00012: ;
    rdfs:comment "Division 5 Partnerships unincorporated associations and trusts - Abrievated Graph Key: D650"@en-AU ;
    skos:broader C2020A00012:651,
        C2020A00012:652,
        C2020A00012:653 ;
    skos:definition "Division 5 Partnerships unincorporated associations and trusts"@en-AU ;
    skos:narrower C2020A00012:633 ;
    skos:prefLabel "Division D650"@en-AU ;
    dcat:accessURL <https://www.legislation.gov.au/C2020A00012/2024-07-10/2024-07-10/text/original/epub/OEBPS/document_1/document_1.html#_Toc172119342> ;
    dcat:landingPage "https://www.legislation.gov.au/C2020A00012/2024-07-10/2024-07-10/text/original/epub/OEBPS/document_1/document_1.html#_Toc172119342"^^xsd:anyURI ;
    dcat:theme legcons:Division .

C2020A00012:82 a legcons:Division,
        owl:Class,
        dcat:Resource ;
    rdfs:label "Division - D82 Division 2 Rule making powers"@en-AU ;
    dct:hasPart C2020A00012:83,
        C2020A00012:84,
        C2020A00012:85 ;
    dct:isPartOf C2020A00012:27 ;
    dct:isReferencedBy C2020A00012: ;
    rdfs:comment "Division 2 Rule making powers - Abrievated Graph Key: D82"@en-AU ;
    skos:broader C2020A00012:83,
        C2020A00012:84,
        C2020A00012:85 ;
    skos:definition "Division 2 Rule making powers"@en-AU ;
    skos:narrower C2020A00012:27 ;
    skos:prefLabel "Division D82"@en-AU ;
    dcat:accessURL <https://www.legislation.gov.au/C2020A00012/2024-07-10/2024-07-10/text/original/epub/OEBPS/document_1/document_1.html#_Toc172118774> ;
    dcat:landingPage "https://www.legislation.gov.au/C2020A00012/2024-07-10/2024-07-10/text/original/epub/OEBPS/document_1/document_1.html#_Toc172118774"^^xsd:anyURI ;
    dcat:theme legcons:Division .

C2020A00012:109 a legcons:Part,
        owl:Class,
        dcat:Resource ;
    rdfs:label "Part - P109 Part 3 Renewal of accreditation"@en-AU ;
    dct:hasPart C2020A00012:110,
        C2020A00012:111,
        C2020A00012:112,
        C2020A00012:113 ;
    dct:isPartOf C2020A00012:100 ;
    dct:isReferencedBy C2020A00012: ;
    rdfs:comment "Part 3 Renewal of accreditation - Abrievated Graph Key: P109"@en-AU ;
    skos:broader C2020A00012:110,
        C2020A00012:111,
        C2020A00012:112,
        C2020A00012:113 ;
    skos:definition "Part 3 Renewal of accreditation"@en-AU ;
    skos:narrower C2020A00012:100 ;
    skos:prefLabel "Part P109"@en-AU ;
    dcat:accessURL <https://www.legislation.gov.au/C2020A00012/2024-07-10/2024-07-10/text/original/epub/OEBPS/document_1/document_1.html#_Toc172118801> ;
    dcat:landingPage "https://www.legislation.gov.au/C2020A00012/2024-07-10/2024-07-10/text/original/epub/OEBPS/document_1/document_1.html#_Toc172118801"^^xsd:anyURI ;
    dcat:theme legcons:Part .

C2020A00012:144 a legcons:Part,
        owl:Class,
        dcat:Resource ;
    rdfs:label "Part - P144 Part 7 Obligations of managers of accredited properties etc"@en-AU ;
    dct:hasPart C2020A00012:145,
        C2020A00012:146,
        C2020A00012:147,
        C2020A00012:148 ;
    dct:isPartOf C2020A00012:100 ;
    dct:isReferencedBy C2020A00012: ;
    rdfs:comment "Part 7 Obligations of managers of accredited properties etc - Abrievated Graph Key: P144"@en-AU ;
    skos:broader C2020A00012:145,
        C2020A00012:146,
        C2020A00012:147,
        C2020A00012:148 ;
    skos:definition "Part 7 Obligations of managers of accredited properties etc"@en-AU ;
    skos:narrower C2020A00012:100 ;
    skos:prefLabel "Part P144"@en-AU ;
    dcat:accessURL <https://www.legislation.gov.au/C2020A00012/2024-07-10/2024-07-10/text/original/epub/OEBPS/document_1/document_1.html#_Toc172118836> ;
    dcat:landingPage "https://www.legislation.gov.au/C2020A00012/2024-07-10/2024-07-10/text/original/epub/OEBPS/document_1/document_1.html#_Toc172118836"^^xsd:anyURI ;
    dcat:theme legcons:Part .

C2020A00012:158 a legcons:Part,
        owl:Class,
        dcat:Resource ;
    rdfs:label "Part - P158 Part 3 Renewal of registration"@en-AU ;
    dct:hasPart C2020A00012:159,
        C2020A00012:160,
        C2020A00012:161,
        C2020A00012:162 ;
    dct:isPartOf C2020A00012:149 ;
    dct:isReferencedBy C2020A00012: ;
    rdfs:comment "Part 3 Renewal of registration - Abrievated Graph Key: P158"@en-AU ;
    skos:broader C2020A00012:159,
        C2020A00012:160,
        C2020A00012:161,
        C2020A00012:162 ;
    skos:definition "Part 3 Renewal of registration"@en-AU ;
    skos:narrower C2020A00012:149 ;
    skos:prefLabel "Part P158"@en-AU ;
    dcat:accessURL <https://www.legislation.gov.au/C2020A00012/2024-07-10/2024-07-10/text/original/epub/OEBPS/document_1/document_1.html#_Toc172118850> ;
    dcat:landingPage "https://www.legislation.gov.au/C2020A00012/2024-07-10/2024-07-10/text/original/epub/OEBPS/document_1/document_1.html#_Toc172118850"^^xsd:anyURI ;
    dcat:theme legcons:Part .

C2020A00012:171 a legcons:Part,
        owl:Class,
        dcat:Resource ;
    rdfs:label "Part - P171 Part 5 Suspension of registration"@en-AU ;
    dct:hasPart C2020A00012:172,
        C2020A00012:175,
        C2020A00012:181,
        C2020A00012:185 ;
    dct:isPartOf C2020A00012:149 ;
    dct:isReferencedBy C2020A00012: ;
    rdfs:comment "Part 5 Suspension of registration - Abrievated Graph Key: P171"@en-AU ;
    skos:broader C2020A00012:172,
        C2020A00012:175,
        C2020A00012:181,
        C2020A00012:185 ;
    skos:definition "Part 5 Suspension of registration"@en-AU ;
    skos:narrower C2020A00012:149 ;
    skos:prefLabel "Part P171"@en-AU ;
    dcat:accessURL <https://www.legislation.gov.au/C2020A00012/2024-07-10/2024-07-10/text/original/epub/OEBPS/document_1/document_1.html#_Toc172118863> ;
    dcat:landingPage "https://www.legislation.gov.au/C2020A00012/2024-07-10/2024-07-10/text/original/epub/OEBPS/document_1/document_1.html#_Toc172118863"^^xsd:anyURI ;
    dcat:theme legcons:Part .

C2020A00012:215 a legcons:Part,
        owl:Class,
        dcat:Resource ;
    rdfs:label "Part - P215 Part 3 Renewal of approved arrangement"@en-AU ;
    dct:hasPart C2020A00012:216,
        C2020A00012:217,
        C2020A00012:218,
        C2020A00012:219 ;
    dct:isPartOf C2020A00012:206 ;
    dct:isReferencedBy C2020A00012: ;
    rdfs:comment "Part 3 Renewal of approved arrangement - Abrievated Graph Key: P215"@en-AU ;
    skos:broader C2020A00012:216,
        C2020A00012:217,
        C2020A00012:218,
        C2020A00012:219 ;
    skos:definition "Part 3 Renewal of approved arrangement"@en-AU ;
    skos:narrower C2020A00012:206 ;
    skos:prefLabel "Part P215"@en-AU ;
    dcat:accessURL <https://www.legislation.gov.au/C2020A00012/2024-07-10/2024-07-10/text/original/epub/OEBPS/document_1/document_1.html#_Toc172118907> ;
    dcat:landingPage "https://www.legislation.gov.au/C2020A00012/2024-07-10/2024-07-10/text/original/epub/OEBPS/document_1/document_1.html#_Toc172118907"^^xsd:anyURI ;
    dcat:theme legcons:Part .

C2020A00012:231 a legcons:Division,
        owl:Class,
        dcat:Resource ;
    rdfs:label "Division - D231 Division 2 Variation required or made by Secretary"@en-AU ;
    dct:hasPart C2020A00012:232,
        C2020A00012:233,
        C2020A00012:234,
        C2020A00012:235 ;
    dct:isPartOf C2020A00012:220 ;
    dct:isReferencedBy C2020A00012: ;
    rdfs:comment "Division 2 Variation required or made by Secretary - Abrievated Graph Key: D231"@en-AU ;
    skos:broader C2020A00012:232,
        C2020A00012:233,
        C2020A00012:234,
        C2020A00012:235 ;
    skos:definition "Division 2 Variation required or made by Secretary"@en-AU ;
    skos:narrower C2020A00012:220 ;
    skos:prefLabel "Division D231"@en-AU ;
    dcat:accessURL <https://www.legislation.gov.au/C2020A00012/2024-07-10/2024-07-10/text/original/epub/OEBPS/document_1/document_1.html#_Toc172118923> ;
    dcat:landingPage "https://www.legislation.gov.au/C2020A00012/2024-07-10/2024-07-10/text/original/epub/OEBPS/document_1/document_1.html#_Toc172118923"^^xsd:anyURI ;
    dcat:theme legcons:Division .

C2020A00012:274 a legcons:Part,
        owl:Class,
        dcat:Resource ;
    rdfs:label "Part - P274 Part 3 Renewal of export licence"@en-AU ;
    dct:hasPart C2020A00012:275,
        C2020A00012:276,
        C2020A00012:277,
        C2020A00012:278 ;
    dct:isPartOf C2020A00012:265 ;
    dct:isReferencedBy C2020A00012: ;
    rdfs:comment "Part 3 Renewal of export licence - Abrievated Graph Key: P274"@en-AU ;
    skos:broader C2020A00012:275,
        C2020A00012:276,
        C2020A00012:277,
        C2020A00012:278 ;
    skos:definition "Part 3 Renewal of export licence"@en-AU ;
    skos:narrower C2020A00012:265 ;
    skos:prefLabel "Part P274"@en-AU ;
    dcat:accessURL <https://www.legislation.gov.au/C2020A00012/2024-07-10/2024-07-10/text/original/epub/OEBPS/document_1/document_1.html#_Toc172118966> ;
    dcat:landingPage "https://www.legislation.gov.au/C2020A00012/2024-07-10/2024-07-10/text/original/epub/OEBPS/document_1/document_1.html#_Toc172118966"^^xsd:anyURI ;
    dcat:theme legcons:Part .

C2020A00012:316 a legcons:Chapter,
        owl:Class,
        dcat:Resource ;
    rdfs:label "Chapter - C316 Chapter 7 Export permits"@en-AU ;
    dct:hasPart C2020A00012:317,
        C2020A00012:319,
        C2020A00012:325,
        C2020A00012:331,
        C2020A00012:336 ;
    dct:isReferencedBy C2020A00012: ;
    rdfs:comment "Chapter 7 Export permits - Abrievated Graph Key: C316"@en-AU ;
    skos:broader C2020A00012:317,
        C2020A00012:319,
        C2020A00012:325,
        C2020A00012:331,
        C2020A00012:336 ;
    skos:definition "Chapter 7 Export permits"@en-AU ;
    skos:prefLabel "Chapter C316"@en-AU ;
    dcat:accessURL <https://www.legislation.gov.au/C2020A00012/2024-07-10/2024-07-10/text/original/epub/OEBPS/document_1/document_1.html#_Toc172119008> ;
    dcat:landingPage "https://www.legislation.gov.au/C2020A00012/2024-07-10/2024-07-10/text/original/epub/OEBPS/document_1/document_1.html#_Toc172119008"^^xsd:anyURI ;
    dcat:theme legcons:Chapter .

C2020A00012:331 a legcons:Part,
        owl:Class,
        dcat:Resource ;
    rdfs:label "Part - P331 Part 4 Other matters"@en-AU ;
    dct:hasPart C2020A00012:332,
        C2020A00012:333,
        C2020A00012:334,
        C2020A00012:335 ;
    dct:isPartOf C2020A00012:316 ;
    dct:isReferencedBy C2020A00012: ;
    rdfs:comment "Part 4 Other matters - Abrievated Graph Key: P331"@en-AU ;
    skos:broader C2020A00012:332,
        C2020A00012:333,
        C2020A00012:334,
        C2020A00012:335 ;
    skos:definition "Part 4 Other matters"@en-AU ;
    skos:narrower C2020A00012:316 ;
    skos:prefLabel "Part P331"@en-AU ;
    dcat:accessURL <https://www.legislation.gov.au/C2020A00012/2024-07-10/2024-07-10/text/original/epub/OEBPS/document_1/document_1.html#_Toc172119023> ;
    dcat:landingPage "https://www.legislation.gov.au/C2020A00012/2024-07-10/2024-07-10/text/original/epub/OEBPS/document_1/document_1.html#_Toc172119023"^^xsd:anyURI ;
    dcat:theme legcons:Part .

C2020A00012:336 a legcons:Part,
        owl:Class,
        dcat:Resource ;
    rdfs:label "Part - P336 Part 5 Applications for export permits"@en-AU ;
    dct:hasPart C2020A00012:337,
        C2020A00012:338,
        C2020A00012:339,
        C2020A00012:340 ;
    dct:isPartOf C2020A00012:316 ;
    dct:isReferencedBy C2020A00012: ;
    rdfs:comment "Part 5 Applications for export permits - Abrievated Graph Key: P336"@en-AU ;
    skos:broader C2020A00012:337,
        C2020A00012:338,
        C2020A00012:339,
        C2020A00012:340 ;
    skos:definition "Part 5 Applications for export permits"@en-AU ;
    skos:narrower C2020A00012:316 ;
    skos:prefLabel "Part P336"@en-AU ;
    dcat:accessURL <https://www.legislation.gov.au/C2020A00012/2024-07-10/2024-07-10/text/original/epub/OEBPS/document_1/document_1.html#_Toc172119028> ;
    dcat:landingPage "https://www.legislation.gov.au/C2020A00012/2024-07-10/2024-07-10/text/original/epub/OEBPS/document_1/document_1.html#_Toc172119028"^^xsd:anyURI ;
    dcat:theme legcons:Part .

C2020A00012:379 a legcons:Chapter,
        owl:Class,
        dcat:Resource ;
    rdfs:label "Chapter - C379 Chapter 9 Powers and officials"@en-AU ;
    dct:hasPart C2020A00012:380,
        C2020A00012:395,
        C2020A00012:407,
        C2020A00012:416,
        C2020A00012:449 ;
    dct:isReferencedBy C2020A00012: ;
    rdfs:comment "Chapter 9 Powers and officials - Abrievated Graph Key: C379"@en-AU ;
    skos:broader C2020A00012:380,
        C2020A00012:395,
        C2020A00012:407,
        C2020A00012:416,
        C2020A00012:449 ;
    skos:definition "Chapter 9 Powers and officials"@en-AU ;
    skos:prefLabel "Chapter C379"@en-AU ;
    dcat:accessURL <https://www.legislation.gov.au/C2020A00012/2024-07-10/2024-07-10/text/original/epub/OEBPS/document_1/document_1.html#_Toc172119071> ;
    dcat:landingPage "https://www.legislation.gov.au/C2020A00012/2024-07-10/2024-07-10/text/original/epub/OEBPS/document_1/document_1.html#_Toc172119071"^^xsd:anyURI ;
    dcat:theme legcons:Chapter .

C2020A00012:398 a legcons:Division,
        owl:Class,
        dcat:Resource ;
    rdfs:label "Division - D398 Division 2 General"@en-AU ;
    dct:hasPart C2020A00012:399,
        C2020A00012:400,
        C2020A00012:401,
        C2020A00012:402 ;
    dct:isPartOf C2020A00012:395 ;
    dct:isReferencedBy C2020A00012: ;
    rdfs:comment "Division 2 General - Abrievated Graph Key: D398"@en-AU ;
    skos:broader C2020A00012:399,
        C2020A00012:400,
        C2020A00012:401,
        C2020A00012:402 ;
    skos:definition "Division 2 General"@en-AU ;
    skos:narrower C2020A00012:395 ;
    skos:prefLabel "Division D398"@en-AU ;
    dcat:accessURL <https://www.legislation.gov.au/C2020A00012/2024-07-10/2024-07-10/text/original/epub/OEBPS/document_1/document_1.html#_Toc172119090> ;
    dcat:landingPage "https://www.legislation.gov.au/C2020A00012/2024-07-10/2024-07-10/text/original/epub/OEBPS/document_1/document_1.html#_Toc172119090"^^xsd:anyURI ;
    dcat:theme legcons:Division .

C2020A00012:419 a legcons:Division,
        owl:Class,
        dcat:Resource ;
    rdfs:label "Division - D419 Division 2 Authorisation"@en-AU ;
    dct:hasPart C2020A00012:420,
        C2020A00012:421,
        C2020A00012:422,
        C2020A00012:423 ;
    dct:isPartOf C2020A00012:416 ;
    dct:isReferencedBy C2020A00012: ;
    rdfs:comment "Division 2 Authorisation - Abrievated Graph Key: D419"@en-AU ;
    skos:broader C2020A00012:420,
        C2020A00012:421,
        C2020A00012:422,
        C2020A00012:423 ;
    skos:definition "Division 2 Authorisation"@en-AU ;
    skos:narrower C2020A00012:416 ;
    skos:prefLabel "Division D419"@en-AU ;
    dcat:accessURL <https://www.legislation.gov.au/C2020A00012/2024-07-10/2024-07-10/text/original/epub/OEBPS/document_1/document_1.html#_Toc172119111> ;
    dcat:landingPage "https://www.legislation.gov.au/C2020A00012/2024-07-10/2024-07-10/text/original/epub/OEBPS/document_1/document_1.html#_Toc172119111"^^xsd:anyURI ;
    dcat:theme legcons:Division .

C2020A00012:425 a legcons:Subdivision,
        owl:Class,
        dcat:Resource ;
    rdfs:label "Subdivision - S425 Subdivision AVariation suspension and revocation on Secretarys own initiative"@en-AU ;
    dct:hasPart C2020A00012:426,
        C2020A00012:427,
        C2020A00012:428,
        C2020A00012:429 ;
    dct:isPartOf C2020A00012:424 ;
    dct:isReferencedBy C2020A00012: ;
    rdfs:comment "Subdivision AVariation suspension and revocation on Secretarys own initiative - Abrievated Graph Key: S425"@en-AU ;
    skos:broader C2020A00012:426,
        C2020A00012:427,
        C2020A00012:428,
        C2020A00012:429 ;
    skos:definition "Subdivision AVariation suspension and revocation on Secretarys own initiative"@en-AU ;
    skos:narrower C2020A00012:424 ;
    skos:prefLabel "Subdivision S425"@en-AU ;
    dcat:accessURL <https://www.legislation.gov.au/C2020A00012/2024-07-10/2024-07-10/text/original/epub/OEBPS/document_1/document_1.html#_Toc172119117> ;
    dcat:landingPage "https://www.legislation.gov.au/C2020A00012/2024-07-10/2024-07-10/text/original/epub/OEBPS/document_1/document_1.html#_Toc172119117"^^xsd:anyURI ;
    dcat:theme legcons:Subdivision .

C2020A00012:430 a legcons:Subdivision,
        owl:Class,
        dcat:Resource ;
    rdfs:label "Subdivision - S430 Subdivision BVariation suspension and revocation on application or request by third party authorised officer"@en-AU ;
    dct:hasPart C2020A00012:431,
        C2020A00012:432,
        C2020A00012:433,
        C2020A00012:434 ;
    dct:isPartOf C2020A00012:424 ;
    dct:isReferencedBy C2020A00012: ;
    rdfs:comment "Subdivision BVariation suspension and revocation on application or request by third party authorised officer - Abrievated Graph Key: S430"@en-AU ;
    skos:broader C2020A00012:431,
        C2020A00012:432,
        C2020A00012:433,
        C2020A00012:434 ;
    skos:definition "Subdivision BVariation suspension and revocation on application or request by third party authorised officer"@en-AU ;
    skos:narrower C2020A00012:424 ;
    skos:prefLabel "Subdivision S430"@en-AU ;
    dcat:accessURL <https://www.legislation.gov.au/C2020A00012/2024-07-10/2024-07-10/text/original/epub/OEBPS/document_1/document_1.html#_Toc172119122> ;
    dcat:landingPage "https://www.legislation.gov.au/C2020A00012/2024-07-10/2024-07-10/text/original/epub/OEBPS/document_1/document_1.html#_Toc172119122"^^xsd:anyURI ;
    dcat:theme legcons:Subdivision .

C2020A00012:444 a legcons:Division,
        owl:Class,
        dcat:Resource ;
    rdfs:label "Division - D444 Division 5 Miscellaneous"@en-AU ;
    dct:hasPart C2020A00012:445,
        C2020A00012:446,
        C2020A00012:447,
        C2020A00012:448 ;
    dct:isPartOf C2020A00012:416 ;
    dct:isReferencedBy C2020A00012: ;
    rdfs:comment "Division 5 Miscellaneous - Abrievated Graph Key: D444"@en-AU ;
    skos:broader C2020A00012:445,
        C2020A00012:446,
        C2020A00012:447,
        C2020A00012:448 ;
    skos:definition "Division 5 Miscellaneous"@en-AU ;
    skos:narrower C2020A00012:416 ;
    skos:prefLabel "Division D444"@en-AU ;
    dcat:accessURL <https://www.legislation.gov.au/C2020A00012/2024-07-10/2024-07-10/text/original/epub/OEBPS/document_1/document_1.html#_Toc172119136> ;
    dcat:landingPage "https://www.legislation.gov.au/C2020A00012/2024-07-10/2024-07-10/text/original/epub/OEBPS/document_1/document_1.html#_Toc172119136"^^xsd:anyURI ;
    dcat:theme legcons:Division .

C2020A00012:449 a legcons:Part,
        owl:Class,
        dcat:Resource ;
    rdfs:label "Part - P449 Part 5 Accredited veterinarians and approved export programs"@en-AU ;
    dct:hasPart C2020A00012:450,
        C2020A00012:452,
        C2020A00012:457,
        C2020A00012:465 ;
    dct:isPartOf C2020A00012:379 ;
    dct:isReferencedBy C2020A00012: ;
    rdfs:comment "Part 5 Accredited veterinarians and approved export programs - Abrievated Graph Key: P449"@en-AU ;
    skos:broader C2020A00012:450,
        C2020A00012:452,
        C2020A00012:457,
        C2020A00012:465 ;
    skos:definition "Part 5 Accredited veterinarians and approved export programs"@en-AU ;
    skos:narrower C2020A00012:379 ;
    skos:prefLabel "Part P449"@en-AU ;
    dcat:accessURL <https://www.legislation.gov.au/C2020A00012/2024-07-10/2024-07-10/text/original/epub/OEBPS/document_1/document_1.html#_Toc172119141> ;
    dcat:landingPage "https://www.legislation.gov.au/C2020A00012/2024-07-10/2024-07-10/text/original/epub/OEBPS/document_1/document_1.html#_Toc172119141"^^xsd:anyURI ;
    dcat:theme legcons:Part .

C2020A00012:452 a legcons:Division,
        owl:Class,
        dcat:Resource ;
    rdfs:label "Division - D452 Division 2 Approved export programs"@en-AU ;
    dct:hasPart C2020A00012:453,
        C2020A00012:454,
        C2020A00012:455,
        C2020A00012:456 ;
    dct:isPartOf C2020A00012:449 ;
    dct:isReferencedBy C2020A00012: ;
    rdfs:comment "Division 2 Approved export programs - Abrievated Graph Key: D452"@en-AU ;
    skos:broader C2020A00012:453,
        C2020A00012:454,
        C2020A00012:455,
        C2020A00012:456 ;
    skos:definition "Division 2 Approved export programs"@en-AU ;
    skos:narrower C2020A00012:449 ;
    skos:prefLabel "Division D452"@en-AU ;
    dcat:accessURL <https://www.legislation.gov.au/C2020A00012/2024-07-10/2024-07-10/text/original/epub/OEBPS/document_1/document_1.html#_Toc172119144> ;
    dcat:landingPage "https://www.legislation.gov.au/C2020A00012/2024-07-10/2024-07-10/text/original/epub/OEBPS/document_1/document_1.html#_Toc172119144"^^xsd:anyURI ;
    dcat:theme legcons:Division .

C2020A00012:503 a legcons:Part,
        owl:Class,
        dcat:Resource ;
    rdfs:label "Part - P503 Part 5 Entering and exercising powers on premises without a warrant or consent"@en-AU ;
    dct:hasPart C2020A00012:504,
        C2020A00012:507,
        C2020A00012:510,
        C2020A00012:513 ;
    dct:isPartOf C2020A00012:467 ;
    dct:isReferencedBy C2020A00012: ;
    rdfs:comment "Part 5 Entering and exercising powers on premises without a warrant or consent - Abrievated Graph Key: P503"@en-AU ;
    skos:broader C2020A00012:504,
        C2020A00012:507,
        C2020A00012:510,
        C2020A00012:513 ;
    skos:definition "Part 5 Entering and exercising powers on premises without a warrant or consent"@en-AU ;
    skos:narrower C2020A00012:467 ;
    skos:prefLabel "Part P503"@en-AU ;
    dcat:accessURL <https://www.legislation.gov.au/C2020A00012/2024-07-10/2024-07-10/text/original/epub/OEBPS/document_1/document_1.html#_Toc172119195> ;
    dcat:landingPage "https://www.legislation.gov.au/C2020A00012/2024-07-10/2024-07-10/text/original/epub/OEBPS/document_1/document_1.html#_Toc172119195"^^xsd:anyURI ;
    dcat:theme legcons:Part .

C2020A00012:570 a legcons:Division,
        owl:Class,
        dcat:Resource ;
    rdfs:label "Division - D570 Division 2 Matters relating to certain applications"@en-AU ;
    dct:hasPart C2020A00012:571,
        C2020A00012:572,
        C2020A00012:573,
        C2020A00012:574 ;
    dct:isPartOf C2020A00012:567 ;
    dct:isReferencedBy C2020A00012: ;
    rdfs:comment "Division 2 Matters relating to certain applications - Abrievated Graph Key: D570"@en-AU ;
    skos:broader C2020A00012:571,
        C2020A00012:572,
        C2020A00012:573,
        C2020A00012:574 ;
    skos:definition "Division 2 Matters relating to certain applications"@en-AU ;
    skos:narrower C2020A00012:567 ;
    skos:prefLabel "Division D570"@en-AU ;
    dcat:accessURL <https://www.legislation.gov.au/C2020A00012/2024-07-10/2024-07-10/text/original/epub/OEBPS/document_1/document_1.html#_Toc172119262> ;
    dcat:landingPage "https://www.legislation.gov.au/C2020A00012/2024-07-10/2024-07-10/text/original/epub/OEBPS/document_1/document_1.html#_Toc172119262"^^xsd:anyURI ;
    dcat:theme legcons:Division .

C2020A00012:645 a legcons:Division,
        owl:Class,
        dcat:Resource ;
    rdfs:label "Division - D645 Division 4 Damaged and destroyed goods etc"@en-AU ;
    dct:hasPart C2020A00012:646,
        C2020A00012:647,
        C2020A00012:648,
        C2020A00012:649 ;
    dct:isPartOf C2020A00012:633 ;
    dct:isReferencedBy C2020A00012: ;
    rdfs:comment "Division 4 Damaged and destroyed goods etc - Abrievated Graph Key: D645"@en-AU ;
    skos:broader C2020A00012:646,
        C2020A00012:647,
        C2020A00012:648,
        C2020A00012:649 ;
    skos:definition "Division 4 Damaged and destroyed goods etc"@en-AU ;
    skos:narrower C2020A00012:633 ;
    skos:prefLabel "Division D645"@en-AU ;
    dcat:accessURL <https://www.legislation.gov.au/C2020A00012/2024-07-10/2024-07-10/text/original/epub/OEBPS/document_1/document_1.html#_Toc172119337> ;
    dcat:landingPage "https://www.legislation.gov.au/C2020A00012/2024-07-10/2024-07-10/text/original/epub/OEBPS/document_1/document_1.html#_Toc172119337"^^xsd:anyURI ;
    dcat:theme legcons:Division .

C2020A00012:657 a legcons:Subdivision,
        owl:Class,
        dcat:Resource ;
    rdfs:label "Subdivision - S657 Subdivision AArrangements and grants"@en-AU ;
    dct:hasPart C2020A00012:658,
        C2020A00012:659,
        C2020A00012:660,
        C2020A00012:661 ;
    dct:isPartOf C2020A00012:656 ;
    dct:isReferencedBy C2020A00012: ;
    rdfs:comment "Subdivision AArrangements and grants - Abrievated Graph Key: S657"@en-AU ;
    skos:broader C2020A00012:658,
        C2020A00012:659,
        C2020A00012:660,
        C2020A00012:661 ;
    skos:definition "Subdivision AArrangements and grants"@en-AU ;
    skos:narrower C2020A00012:656 ;
    skos:prefLabel "Subdivision S657"@en-AU ;
    dcat:accessURL <https://www.legislation.gov.au/C2020A00012/2024-07-10/2024-07-10/text/original/epub/OEBPS/document_1/document_1.html#_Toc172119349> ;
    dcat:landingPage "https://www.legislation.gov.au/C2020A00012/2024-07-10/2024-07-10/text/original/epub/OEBPS/document_1/document_1.html#_Toc172119349"^^xsd:anyURI ;
    dcat:theme legcons:Subdivision .

C2020A00012:680 a legcons:Endnotes,
        owl:Class,
        dcat:Resource ;
    rdfs:label "Endnotes - E680 Endnotes"@en-AU ;
    dct:hasPart C2020A00012:681,
        C2020A00012:682,
        C2020A00012:683,
        C2020A00012:684 ;
    dct:isPartOf C2020A00012:566 ;
    dct:isReferencedBy C2020A00012: ;
    rdfs:comment "Endnotes - Abrievated Graph Key: E680"@en-AU ;
    skos:broader C2020A00012:681,
        C2020A00012:682,
        C2020A00012:683,
        C2020A00012:684 ;
    skos:definition "Endnotes"@en-AU ;
    skos:narrower C2020A00012:566 ;
    skos:prefLabel "Endnotes E680"@en-AU ;
    dcat:accessURL <https://www.legislation.gov.au/C2020A00012/2024-07-10/2024-07-10/text/original/epub/OEBPS/document_1/document_1.html#_Toc172119372> ;
    dcat:landingPage "https://www.legislation.gov.au/C2020A00012/2024-07-10/2024-07-10/text/original/epub/OEBPS/document_1/document_1.html#_Toc172119372"^^xsd:anyURI ;
    dcat:theme legcons:Endnotes .

C2020A00012:95 a legcons:Division,
        owl:Class,
        dcat:Resource ;
    rdfs:label "Division - D95 Division 4 Other matters"@en-AU ;
    dct:hasPart C2020A00012:96,
        C2020A00012:97,
        C2020A00012:98,
        C2020A00012:99 ;
    dct:isPartOf C2020A00012:27 ;
    dct:isReferencedBy C2020A00012: ;
    rdfs:comment "Division 4 Other matters - Abrievated Graph Key: D95"@en-AU ;
    skos:broader C2020A00012:96,
        C2020A00012:97,
        C2020A00012:98,
        C2020A00012:99 ;
    skos:definition "Division 4 Other matters"@en-AU ;
    skos:narrower C2020A00012:27 ;
    skos:prefLabel "Division D95"@en-AU ;
    dcat:accessURL <https://www.legislation.gov.au/C2020A00012/2024-07-10/2024-07-10/text/original/epub/OEBPS/document_1/document_1.html#_Toc172118787> ;
    dcat:landingPage "https://www.legislation.gov.au/C2020A00012/2024-07-10/2024-07-10/text/original/epub/OEBPS/document_1/document_1.html#_Toc172118787"^^xsd:anyURI ;
    dcat:theme legcons:Division .

C2020A00012:103 a legcons:Part,
        owl:Class,
        dcat:Resource ;
    rdfs:label "Part - P103 Part 2 Application for accreditation"@en-AU ;
    dct:hasPart C2020A00012:104,
        C2020A00012:105,
        C2020A00012:106,
        C2020A00012:107,
        C2020A00012:108 ;
    dct:isPartOf C2020A00012:100 ;
    dct:isReferencedBy C2020A00012: ;
    rdfs:comment "Part 2 Application for accreditation - Abrievated Graph Key: P103"@en-AU ;
    skos:broader C2020A00012:104,
        C2020A00012:105,
        C2020A00012:106,
        C2020A00012:107,
        C2020A00012:108 ;
    skos:definition "Part 2 Application for accreditation"@en-AU ;
    skos:narrower C2020A00012:100 ;
    skos:prefLabel "Part P103"@en-AU ;
    dcat:accessURL <https://www.legislation.gov.au/C2020A00012/2024-07-10/2024-07-10/text/original/epub/OEBPS/document_1/document_1.html#_Toc172118795> ;
    dcat:landingPage "https://www.legislation.gov.au/C2020A00012/2024-07-10/2024-07-10/text/original/epub/OEBPS/document_1/document_1.html#_Toc172118795"^^xsd:anyURI ;
    dcat:theme legcons:Part .

C2020A00012:126 a legcons:Division,
        owl:Class,
        dcat:Resource ;
    rdfs:label "Division - D126 Division 2 Suspension by Secretary"@en-AU ;
    dct:hasPart C2020A00012:127,
        C2020A00012:128,
        C2020A00012:129,
        C2020A00012:130,
        C2020A00012:131 ;
    dct:isPartOf C2020A00012:122 ;
    dct:isReferencedBy C2020A00012: ;
    rdfs:comment "Division 2 Suspension by Secretary - Abrievated Graph Key: D126"@en-AU ;
    skos:broader C2020A00012:127,
        C2020A00012:128,
        C2020A00012:129,
        C2020A00012:130,
        C2020A00012:131 ;
    skos:definition "Division 2 Suspension by Secretary"@en-AU ;
    skos:narrower C2020A00012:122 ;
    skos:prefLabel "Division D126"@en-AU ;
    dcat:accessURL <https://www.legislation.gov.au/C2020A00012/2024-07-10/2024-07-10/text/original/epub/OEBPS/document_1/document_1.html#_Toc172118818> ;
    dcat:landingPage "https://www.legislation.gov.au/C2020A00012/2024-07-10/2024-07-10/text/original/epub/OEBPS/document_1/document_1.html#_Toc172118818"^^xsd:anyURI ;
    dcat:theme legcons:Division .

C2020A00012:152 a legcons:Part,
        owl:Class,
        dcat:Resource ;
    rdfs:label "Part - P152 Part 2 Application for registration"@en-AU ;
    dct:hasPart C2020A00012:153,
        C2020A00012:154,
        C2020A00012:155,
        C2020A00012:156,
        C2020A00012:157 ;
    dct:isPartOf C2020A00012:149 ;
    dct:isReferencedBy C2020A00012: ;
    rdfs:comment "Part 2 Application for registration - Abrievated Graph Key: P152"@en-AU ;
    skos:broader C2020A00012:153,
        C2020A00012:154,
        C2020A00012:155,
        C2020A00012:156,
        C2020A00012:157 ;
    skos:definition "Part 2 Application for registration"@en-AU ;
    skos:narrower C2020A00012:149 ;
    skos:prefLabel "Part P152"@en-AU ;
    dcat:accessURL <https://www.legislation.gov.au/C2020A00012/2024-07-10/2024-07-10/text/original/epub/OEBPS/document_1/document_1.html#_Toc172118844> ;
    dcat:landingPage "https://www.legislation.gov.au/C2020A00012/2024-07-10/2024-07-10/text/original/epub/OEBPS/document_1/document_1.html#_Toc172118844"^^xsd:anyURI ;
    dcat:theme legcons:Part .

C2020A00012:175 a legcons:Division,
        owl:Class,
        dcat:Resource ;
    rdfs:label "Division - D175 Division 2 Suspension by Secretary"@en-AU ;
    dct:hasPart C2020A00012:176,
        C2020A00012:177,
        C2020A00012:178,
        C2020A00012:179,
        C2020A00012:180 ;
    dct:isPartOf C2020A00012:171 ;
    dct:isReferencedBy C2020A00012: ;
    rdfs:comment "Division 2 Suspension by Secretary - Abrievated Graph Key: D175"@en-AU ;
    skos:broader C2020A00012:176,
        C2020A00012:177,
        C2020A00012:178,
        C2020A00012:179,
        C2020A00012:180 ;
    skos:definition "Division 2 Suspension by Secretary"@en-AU ;
    skos:narrower C2020A00012:171 ;
    skos:prefLabel "Division D175"@en-AU ;
    dcat:accessURL <https://www.legislation.gov.au/C2020A00012/2024-07-10/2024-07-10/text/original/epub/OEBPS/document_1/document_1.html#_Toc172118867> ;
    dcat:landingPage "https://www.legislation.gov.au/C2020A00012/2024-07-10/2024-07-10/text/original/epub/OEBPS/document_1/document_1.html#_Toc172118867"^^xsd:anyURI ;
    dcat:theme legcons:Division .

C2020A00012:198 a legcons:Part,
        owl:Class,
        dcat:Resource ;
    rdfs:label "Part - P198 Part 7 Obligations of occupiers of registered establishments"@en-AU ;
    dct:hasPart C2020A00012:199,
        C2020A00012:200,
        C2020A00012:201,
        C2020A00012:202,
        C2020A00012:203 ;
    dct:isPartOf C2020A00012:149 ;
    dct:isReferencedBy C2020A00012: ;
    rdfs:comment "Part 7 Obligations of occupiers of registered establishments - Abrievated Graph Key: P198"@en-AU ;
    skos:broader C2020A00012:199,
        C2020A00012:200,
        C2020A00012:201,
        C2020A00012:202,
        C2020A00012:203 ;
    skos:definition "Part 7 Obligations of occupiers of registered establishments"@en-AU ;
    skos:narrower C2020A00012:149 ;
    skos:prefLabel "Part P198"@en-AU ;
    dcat:accessURL <https://www.legislation.gov.au/C2020A00012/2024-07-10/2024-07-10/text/original/epub/OEBPS/document_1/document_1.html#_Toc172118890> ;
    dcat:landingPage "https://www.legislation.gov.au/C2020A00012/2024-07-10/2024-07-10/text/original/epub/OEBPS/document_1/document_1.html#_Toc172118890"^^xsd:anyURI ;
    dcat:theme legcons:Part .

C2020A00012:209 a legcons:Part,
        owl:Class,
        dcat:Resource ;
    rdfs:label "Part - P209 Part 2 Approval of proposed arrangement"@en-AU ;
    dct:hasPart C2020A00012:210,
        C2020A00012:211,
        C2020A00012:212,
        C2020A00012:213,
        C2020A00012:214 ;
    dct:isPartOf C2020A00012:206 ;
    dct:isReferencedBy C2020A00012: ;
    rdfs:comment "Part 2 Approval of proposed arrangement - Abrievated Graph Key: P209"@en-AU ;
    skos:broader C2020A00012:210,
        C2020A00012:211,
        C2020A00012:212,
        C2020A00012:213,
        C2020A00012:214 ;
    skos:definition "Part 2 Approval of proposed arrangement"@en-AU ;
    skos:narrower C2020A00012:206 ;
    skos:prefLabel "Part P209"@en-AU ;
    dcat:accessURL <https://www.legislation.gov.au/C2020A00012/2024-07-10/2024-07-10/text/original/epub/OEBPS/document_1/document_1.html#_Toc172118901> ;
    dcat:landingPage "https://www.legislation.gov.au/C2020A00012/2024-07-10/2024-07-10/text/original/epub/OEBPS/document_1/document_1.html#_Toc172118901"^^xsd:anyURI ;
    dcat:theme legcons:Part .

C2020A00012:240 a legcons:Division,
        owl:Class,
        dcat:Resource ;
    rdfs:label "Division - D240 Division 2 Suspension by Secretary"@en-AU ;
    dct:hasPart C2020A00012:241,
        C2020A00012:242,
        C2020A00012:243,
        C2020A00012:244,
        C2020A00012:245 ;
    dct:isPartOf C2020A00012:236 ;
    dct:isReferencedBy C2020A00012: ;
    rdfs:comment "Division 2 Suspension by Secretary - Abrievated Graph Key: D240"@en-AU ;
    skos:broader C2020A00012:241,
        C2020A00012:242,
        C2020A00012:243,
        C2020A00012:244,
        C2020A00012:245 ;
    skos:definition "Division 2 Suspension by Secretary"@en-AU ;
    skos:narrower C2020A00012:236 ;
    skos:prefLabel "Division D240"@en-AU ;
    dcat:accessURL <https://www.legislation.gov.au/C2020A00012/2024-07-10/2024-07-10/text/original/epub/OEBPS/document_1/document_1.html#_Toc172118932> ;
    dcat:landingPage "https://www.legislation.gov.au/C2020A00012/2024-07-10/2024-07-10/text/original/epub/OEBPS/document_1/document_1.html#_Toc172118932"^^xsd:anyURI ;
    dcat:theme legcons:Division .

C2020A00012:259 a legcons:Part,
        owl:Class,
        dcat:Resource ;
    rdfs:label "Part - P259 Part 7 Obligations of holders of approved arrangements"@en-AU ;
    dct:hasPart C2020A00012:260,
        C2020A00012:261,
        C2020A00012:262,
        C2020A00012:263,
        C2020A00012:264 ;
    dct:isPartOf C2020A00012:206 ;
    dct:isReferencedBy C2020A00012: ;
    rdfs:comment "Part 7 Obligations of holders of approved arrangements - Abrievated Graph Key: P259"@en-AU ;
    skos:broader C2020A00012:260,
        C2020A00012:261,
        C2020A00012:262,
        C2020A00012:263,
        C2020A00012:264 ;
    skos:definition "Part 7 Obligations of holders of approved arrangements"@en-AU ;
    skos:narrower C2020A00012:206 ;
    skos:prefLabel "Part P259"@en-AU ;
    dcat:accessURL <https://www.legislation.gov.au/C2020A00012/2024-07-10/2024-07-10/text/original/epub/OEBPS/document_1/document_1.html#_Toc172118951> ;
    dcat:landingPage "https://www.legislation.gov.au/C2020A00012/2024-07-10/2024-07-10/text/original/epub/OEBPS/document_1/document_1.html#_Toc172118951"^^xsd:anyURI ;
    dcat:theme legcons:Part .

C2020A00012:268 a legcons:Part,
        owl:Class,
        dcat:Resource ;
    rdfs:label "Part - P268 Part 2 Grant of export licence"@en-AU ;
    dct:hasPart C2020A00012:269,
        C2020A00012:270,
        C2020A00012:271,
        C2020A00012:272,
        C2020A00012:273 ;
    dct:isPartOf C2020A00012:265 ;
    dct:isReferencedBy C2020A00012: ;
    rdfs:comment "Part 2 Grant of export licence - Abrievated Graph Key: P268"@en-AU ;
    skos:broader C2020A00012:269,
        C2020A00012:270,
        C2020A00012:271,
        C2020A00012:272,
        C2020A00012:273 ;
    skos:definition "Part 2 Grant of export licence"@en-AU ;
    skos:narrower C2020A00012:265 ;
    skos:prefLabel "Part P268"@en-AU ;
    dcat:accessURL <https://www.legislation.gov.au/C2020A00012/2024-07-10/2024-07-10/text/original/epub/OEBPS/document_1/document_1.html#_Toc172118960> ;
    dcat:landingPage "https://www.legislation.gov.au/C2020A00012/2024-07-10/2024-07-10/text/original/epub/OEBPS/document_1/document_1.html#_Toc172118960"^^xsd:anyURI ;
    dcat:theme legcons:Part .

C2020A00012:290 a legcons:Division,
        owl:Class,
        dcat:Resource ;
    rdfs:label "Division - D290 Division 2 Suspension by Secretary"@en-AU ;
    dct:hasPart C2020A00012:291,
        C2020A00012:292,
        C2020A00012:293,
        C2020A00012:294,
        C2020A00012:295 ;
    dct:isPartOf C2020A00012:286 ;
    dct:isReferencedBy C2020A00012: ;
    rdfs:comment "Division 2 Suspension by Secretary - Abrievated Graph Key: D290"@en-AU ;
    skos:broader C2020A00012:291,
        C2020A00012:292,
        C2020A00012:293,
        C2020A00012:294,
        C2020A00012:295 ;
    skos:definition "Division 2 Suspension by Secretary"@en-AU ;
    skos:narrower C2020A00012:286 ;
    skos:prefLabel "Division D290"@en-AU ;
    dcat:accessURL <https://www.legislation.gov.au/C2020A00012/2024-07-10/2024-07-10/text/original/epub/OEBPS/document_1/document_1.html#_Toc172118982> ;
    dcat:landingPage "https://www.legislation.gov.au/C2020A00012/2024-07-10/2024-07-10/text/original/epub/OEBPS/document_1/document_1.html#_Toc172118982"^^xsd:anyURI ;
    dcat:theme legcons:Division .

C2020A00012:319 a legcons:Part,
        owl:Class,
        dcat:Resource ;
    rdfs:label "Part - P319 Part 2 Issue of export permit"@en-AU ;
    dct:hasPart C2020A00012:320,
        C2020A00012:321,
        C2020A00012:322,
        C2020A00012:323,
        C2020A00012:324 ;
    dct:isPartOf C2020A00012:316 ;
    dct:isReferencedBy C2020A00012: ;
    rdfs:comment "Part 2 Issue of export permit - Abrievated Graph Key: P319"@en-AU ;
    skos:broader C2020A00012:320,
        C2020A00012:321,
        C2020A00012:322,
        C2020A00012:323,
        C2020A00012:324 ;
    skos:definition "Part 2 Issue of export permit"@en-AU ;
    skos:narrower C2020A00012:316 ;
    skos:prefLabel "Part P319"@en-AU ;
    dcat:accessURL <https://www.legislation.gov.au/C2020A00012/2024-07-10/2024-07-10/text/original/epub/OEBPS/document_1/document_1.html#_Toc172119011> ;
    dcat:landingPage "https://www.legislation.gov.au/C2020A00012/2024-07-10/2024-07-10/text/original/epub/OEBPS/document_1/document_1.html#_Toc172119011"^^xsd:anyURI ;
    dcat:theme legcons:Part .

C2020A00012:325 a legcons:Part,
        owl:Class,
        dcat:Resource ;
    rdfs:label "Part - P325 Part 3 Variation suspension and revocation of export permit"@en-AU ;
    dct:hasPart C2020A00012:326,
        C2020A00012:327,
        C2020A00012:328,
        C2020A00012:329,
        C2020A00012:330 ;
    dct:isPartOf C2020A00012:316 ;
    dct:isReferencedBy C2020A00012: ;
    rdfs:comment "Part 3 Variation suspension and revocation of export permit - Abrievated Graph Key: P325"@en-AU ;
    skos:broader C2020A00012:326,
        C2020A00012:327,
        C2020A00012:328,
        C2020A00012:329,
        C2020A00012:330 ;
    skos:definition "Part 3 Variation suspension and revocation of export permit"@en-AU ;
    skos:narrower C2020A00012:316 ;
    skos:prefLabel "Part P325"@en-AU ;
    dcat:accessURL <https://www.legislation.gov.au/C2020A00012/2024-07-10/2024-07-10/text/original/epub/OEBPS/document_1/document_1.html#_Toc172119017> ;
    dcat:landingPage "https://www.legislation.gov.au/C2020A00012/2024-07-10/2024-07-10/text/original/epub/OEBPS/document_1/document_1.html#_Toc172119017"^^xsd:anyURI ;
    dcat:theme legcons:Part .

C2020A00012:351 a legcons:Division,
        owl:Class,
        dcat:Resource ;
    rdfs:label "Division - D351 Division 2 Trade descriptions for prescribed goods"@en-AU ;
    dct:hasPart C2020A00012:352,
        C2020A00012:353,
        C2020A00012:354,
        C2020A00012:355,
        C2020A00012:356 ;
    dct:isPartOf C2020A00012:348 ;
    dct:isReferencedBy C2020A00012: ;
    rdfs:comment "Division 2 Trade descriptions for prescribed goods - Abrievated Graph Key: D351"@en-AU ;
    skos:broader C2020A00012:352,
        C2020A00012:353,
        C2020A00012:354,
        C2020A00012:355,
        C2020A00012:356 ;
    skos:definition "Division 2 Trade descriptions for prescribed goods"@en-AU ;
    skos:narrower C2020A00012:348 ;
    skos:prefLabel "Division D351"@en-AU ;
    dcat:accessURL <https://www.legislation.gov.au/C2020A00012/2024-07-10/2024-07-10/text/original/epub/OEBPS/document_1/document_1.html#_Toc172119043> ;
    dcat:landingPage "https://www.legislation.gov.au/C2020A00012/2024-07-10/2024-07-10/text/original/epub/OEBPS/document_1/document_1.html#_Toc172119043"^^xsd:anyURI ;
    dcat:theme legcons:Division .

C2020A00012:368 a legcons:Division,
        owl:Class,
        dcat:Resource ;
    rdfs:label "Division - D368 Division 3 Offences and civil penalty provisions"@en-AU ;
    dct:hasPart C2020A00012:369,
        C2020A00012:370,
        C2020A00012:371,
        C2020A00012:372,
        C2020A00012:373 ;
    dct:isPartOf C2020A00012:361 ;
    dct:isReferencedBy C2020A00012: ;
    rdfs:comment "Division 3 Offences and civil penalty provisions - Abrievated Graph Key: D368"@en-AU ;
    skos:broader C2020A00012:369,
        C2020A00012:370,
        C2020A00012:371,
        C2020A00012:372,
        C2020A00012:373 ;
    skos:definition "Division 3 Offences and civil penalty provisions"@en-AU ;
    skos:narrower C2020A00012:361 ;
    skos:prefLabel "Division D368"@en-AU ;
    dcat:accessURL <https://www.legislation.gov.au/C2020A00012/2024-07-10/2024-07-10/text/original/epub/OEBPS/document_1/document_1.html#_Toc172119060> ;
    dcat:landingPage "https://www.legislation.gov.au/C2020A00012/2024-07-10/2024-07-10/text/original/epub/OEBPS/document_1/document_1.html#_Toc172119060"^^xsd:anyURI ;
    dcat:theme legcons:Division .

C2020A00012:410 a legcons:Division,
        owl:Class,
        dcat:Resource ;
    rdfs:label "Division - D410 Division 2 Powers of the Secretary"@en-AU ;
    dct:hasPart C2020A00012:411,
        C2020A00012:412,
        C2020A00012:413,
        C2020A00012:414,
        C2020A00012:415 ;
    dct:isPartOf C2020A00012:407 ;
    dct:isReferencedBy C2020A00012: ;
    rdfs:comment "Division 2 Powers of the Secretary - Abrievated Graph Key: D410"@en-AU ;
    skos:broader C2020A00012:411,
        C2020A00012:412,
        C2020A00012:413,
        C2020A00012:414,
        C2020A00012:415 ;
    skos:definition "Division 2 Powers of the Secretary"@en-AU ;
    skos:narrower C2020A00012:407 ;
    skos:prefLabel "Division D410"@en-AU ;
    dcat:accessURL <https://www.legislation.gov.au/C2020A00012/2024-07-10/2024-07-10/text/original/epub/OEBPS/document_1/document_1.html#_Toc172119102> ;
    dcat:landingPage "https://www.legislation.gov.au/C2020A00012/2024-07-10/2024-07-10/text/original/epub/OEBPS/document_1/document_1.html#_Toc172119102"^^xsd:anyURI ;
    dcat:theme legcons:Division .

C2020A00012:416 a legcons:Part,
        owl:Class,
        dcat:Resource ;
    rdfs:label "Part - P416 Part 4 Authorised officers"@en-AU ;
    dct:hasPart C2020A00012:417,
        C2020A00012:419,
        C2020A00012:424,
        C2020A00012:437,
        C2020A00012:444 ;
    dct:isPartOf C2020A00012:379 ;
    dct:isReferencedBy C2020A00012: ;
    rdfs:comment "Part 4 Authorised officers - Abrievated Graph Key: P416"@en-AU ;
    skos:broader C2020A00012:417,
        C2020A00012:419,
        C2020A00012:424,
        C2020A00012:437,
        C2020A00012:444 ;
    skos:definition "Part 4 Authorised officers"@en-AU ;
    skos:narrower C2020A00012:379 ;
    skos:prefLabel "Part P416"@en-AU ;
    dcat:accessURL <https://www.legislation.gov.au/C2020A00012/2024-07-10/2024-07-10/text/original/epub/OEBPS/document_1/document_1.html#_Toc172119108> ;
    dcat:landingPage "https://www.legislation.gov.au/C2020A00012/2024-07-10/2024-07-10/text/original/epub/OEBPS/document_1/document_1.html#_Toc172119108"^^xsd:anyURI ;
    dcat:theme legcons:Part .

C2020A00012:492 a legcons:Division,
        owl:Class,
        dcat:Resource ;
    rdfs:label "Division - D492 Division 4 Obligations and powers of authorised officers"@en-AU ;
    dct:hasPart C2020A00012:493,
        C2020A00012:494,
        C2020A00012:495,
        C2020A00012:496,
        C2020A00012:497 ;
    dct:isPartOf C2020A00012:483 ;
    dct:isReferencedBy C2020A00012: ;
    rdfs:comment "Division 4 Obligations and powers of authorised officers - Abrievated Graph Key: D492"@en-AU ;
    skos:broader C2020A00012:493,
        C2020A00012:494,
        C2020A00012:495,
        C2020A00012:496,
        C2020A00012:497 ;
    skos:definition "Division 4 Obligations and powers of authorised officers"@en-AU ;
    skos:narrower C2020A00012:483 ;
    skos:prefLabel "Division D492"@en-AU ;
    dcat:accessURL <https://www.legislation.gov.au/C2020A00012/2024-07-10/2024-07-10/text/original/epub/OEBPS/document_1/document_1.html#_Toc172119184> ;
    dcat:landingPage "https://www.legislation.gov.au/C2020A00012/2024-07-10/2024-07-10/text/original/epub/OEBPS/document_1/document_1.html#_Toc172119184"^^xsd:anyURI ;
    dcat:theme legcons:Division .

C2020A00012:550 a legcons:Part,
        owl:Class,
        dcat:Resource ;
    rdfs:label "Part - P550 Part 11 Miscellaneous"@en-AU ;
    dct:hasPart C2020A00012:551,
        C2020A00012:553,
        C2020A00012:555,
        C2020A00012:559,
        C2020A00012:562 ;
    dct:isPartOf C2020A00012:467 ;
    dct:isReferencedBy C2020A00012: ;
    rdfs:comment "Part 11 Miscellaneous - Abrievated Graph Key: P550"@en-AU ;
    skos:broader C2020A00012:551,
        C2020A00012:553,
        C2020A00012:555,
        C2020A00012:559,
        C2020A00012:562 ;
    skos:definition "Part 11 Miscellaneous"@en-AU ;
    skos:narrower C2020A00012:467 ;
    skos:prefLabel "Part P550"@en-AU ;
    dcat:accessURL <https://www.legislation.gov.au/C2020A00012/2024-07-10/2024-07-10/text/original/epub/OEBPS/document_1/document_1.html#_Toc172119242> ;
    dcat:landingPage "https://www.legislation.gov.au/C2020A00012/2024-07-10/2024-07-10/text/original/epub/OEBPS/document_1/document_1.html#_Toc172119242"^^xsd:anyURI ;
    dcat:theme legcons:Part .

C2020A00012:613 a legcons:Part,
        owl:Class,
        dcat:Resource ;
    rdfs:label "Part - P613 Part 4 Cost recovery"@en-AU ;
    dct:hasPart C2020A00012:614,
        C2020A00012:616,
        C2020A00012:618,
        C2020A00012:622,
        C2020A00012:625 ;
    dct:isPartOf C2020A00012:566 ;
    dct:isReferencedBy C2020A00012: ;
    rdfs:comment "Part 4 Cost recovery - Abrievated Graph Key: P613"@en-AU ;
    skos:broader C2020A00012:614,
        C2020A00012:616,
        C2020A00012:618,
        C2020A00012:622,
        C2020A00012:625 ;
    skos:definition "Part 4 Cost recovery"@en-AU ;
    skos:narrower C2020A00012:566 ;
    skos:prefLabel "Part P613"@en-AU ;
    dcat:accessURL <https://www.legislation.gov.au/C2020A00012/2024-07-10/2024-07-10/text/original/epub/OEBPS/document_1/document_1.html#_Toc172119305> ;
    dcat:landingPage "https://www.legislation.gov.au/C2020A00012/2024-07-10/2024-07-10/text/original/epub/OEBPS/document_1/document_1.html#_Toc172119305"^^xsd:anyURI ;
    dcat:theme legcons:Part .

C2020A00012:100 a legcons:Chapter,
        owl:Class,
        dcat:Resource ;
    rdfs:label "Chapter - C100 Chapter 3 Accredited properties"@en-AU ;
    dct:hasPart C2020A00012:101,
        C2020A00012:103,
        C2020A00012:109,
        C2020A00012:114,
        C2020A00012:122,
        C2020A00012:135,
        C2020A00012:144 ;
    dct:isReferencedBy C2020A00012: ;
    rdfs:comment "Chapter 3 Accredited properties - Abrievated Graph Key: C100"@en-AU ;
    skos:broader C2020A00012:101,
        C2020A00012:103,
        C2020A00012:109,
        C2020A00012:114,
        C2020A00012:122,
        C2020A00012:135,
        C2020A00012:144 ;
    skos:definition "Chapter 3 Accredited properties"@en-AU ;
    skos:prefLabel "Chapter C100"@en-AU ;
    dcat:accessURL <https://www.legislation.gov.au/C2020A00012/2024-07-10/2024-07-10/text/original/epub/OEBPS/document_1/document_1.html#_Toc172118792> ;
    dcat:landingPage "https://www.legislation.gov.au/C2020A00012/2024-07-10/2024-07-10/text/original/epub/OEBPS/document_1/document_1.html#_Toc172118792"^^xsd:anyURI ;
    dcat:theme legcons:Chapter .

C2020A00012:206 a legcons:Chapter,
        owl:Class,
        dcat:Resource ;
    rdfs:label "Chapter - C206 Chapter 5 Approved arrangements"@en-AU ;
    dct:hasPart C2020A00012:207,
        C2020A00012:209,
        C2020A00012:215,
        C2020A00012:220,
        C2020A00012:236,
        C2020A00012:249,
        C2020A00012:259 ;
    dct:isReferencedBy C2020A00012: ;
    rdfs:comment "Chapter 5 Approved arrangements - Abrievated Graph Key: C206"@en-AU ;
    skos:broader C2020A00012:207,
        C2020A00012:209,
        C2020A00012:215,
        C2020A00012:220,
        C2020A00012:236,
        C2020A00012:249,
        C2020A00012:259 ;
    skos:definition "Chapter 5 Approved arrangements"@en-AU ;
    skos:prefLabel "Chapter C206"@en-AU ;
    dcat:accessURL <https://www.legislation.gov.au/C2020A00012/2024-07-10/2024-07-10/text/original/epub/OEBPS/document_1/document_1.html#_Toc172118898> ;
    dcat:landingPage "https://www.legislation.gov.au/C2020A00012/2024-07-10/2024-07-10/text/original/epub/OEBPS/document_1/document_1.html#_Toc172118898"^^xsd:anyURI ;
    dcat:theme legcons:Chapter .

C2020A00012:31 a legcons:Division,
        owl:Class,
        dcat:Resource ;
    rdfs:label "Division - D31 Division 2 Prohibited goods and exports"@en-AU ;
    dct:hasPart C2020A00012:32,
        C2020A00012:35,
        C2020A00012:36,
        C2020A00012:37,
        C2020A00012:38,
        C2020A00012:39 ;
    dct:isPartOf C2020A00012:28 ;
    dct:isReferencedBy C2020A00012: ;
    rdfs:comment "Division 2 Prohibited goods and exports - Abrievated Graph Key: D31"@en-AU ;
    skos:broader C2020A00012:32,
        C2020A00012:35,
        C2020A00012:36,
        C2020A00012:37,
        C2020A00012:38,
        C2020A00012:39 ;
    skos:definition "Division 2 Prohibited goods and exports"@en-AU ;
    skos:narrower C2020A00012:28 ;
    skos:prefLabel "Division D31"@en-AU ;
    dcat:accessURL <https://www.legislation.gov.au/C2020A00012/2024-07-10/2024-07-10/text/original/epub/OEBPS/document_1/document_1.html#_Toc172118723> ;
    dcat:landingPage "https://www.legislation.gov.au/C2020A00012/2024-07-10/2024-07-10/text/original/epub/OEBPS/document_1/document_1.html#_Toc172118723"^^xsd:anyURI ;
    dcat:theme legcons:Division .

C2020A00012:437 a legcons:Division,
        owl:Class,
        dcat:Resource ;
    rdfs:label "Division - D437 Division 4 Functions and powers"@en-AU ;
    dct:hasPart C2020A00012:438,
        C2020A00012:439,
        C2020A00012:440,
        C2020A00012:441,
        C2020A00012:442,
        C2020A00012:443 ;
    dct:isPartOf C2020A00012:416 ;
    dct:isReferencedBy C2020A00012: ;
    rdfs:comment "Division 4 Functions and powers - Abrievated Graph Key: D437"@en-AU ;
    skos:broader C2020A00012:438,
        C2020A00012:439,
        C2020A00012:440,
        C2020A00012:441,
        C2020A00012:442,
        C2020A00012:443 ;
    skos:definition "Division 4 Functions and powers"@en-AU ;
    skos:narrower C2020A00012:416 ;
    skos:prefLabel "Division D437"@en-AU ;
    dcat:accessURL <https://www.legislation.gov.au/C2020A00012/2024-07-10/2024-07-10/text/original/epub/OEBPS/document_1/document_1.html#_Toc172119129> ;
    dcat:landingPage "https://www.legislation.gov.au/C2020A00012/2024-07-10/2024-07-10/text/original/epub/OEBPS/document_1/document_1.html#_Toc172119129"^^xsd:anyURI ;
    dcat:theme legcons:Division .

C2020A00012:483 a legcons:Part,
        owl:Class,
        dcat:Resource ;
    rdfs:label "Part - P483 Part 4 Entry to adjacent premises"@en-AU ;
    dct:hasPart C2020A00012:484,
        C2020A00012:487,
        C2020A00012:490,
        C2020A00012:492,
        C2020A00012:498,
        C2020A00012:501 ;
    dct:isPartOf C2020A00012:467 ;
    dct:isReferencedBy C2020A00012: ;
    rdfs:comment "Part 4 Entry to adjacent premises - Abrievated Graph Key: P483"@en-AU ;
    skos:broader C2020A00012:484,
        C2020A00012:487,
        C2020A00012:490,
        C2020A00012:492,
        C2020A00012:498,
        C2020A00012:501 ;
    skos:definition "Part 4 Entry to adjacent premises"@en-AU ;
    skos:narrower C2020A00012:467 ;
    skos:prefLabel "Part P483"@en-AU ;
    dcat:accessURL <https://www.legislation.gov.au/C2020A00012/2024-07-10/2024-07-10/text/original/epub/OEBPS/document_1/document_1.html#_Toc172119175> ;
    dcat:landingPage "https://www.legislation.gov.au/C2020A00012/2024-07-10/2024-07-10/text/original/epub/OEBPS/document_1/document_1.html#_Toc172119175"^^xsd:anyURI ;
    dcat:theme legcons:Part .

C2020A00012:543 a legcons:Part,
        owl:Class,
        dcat:Resource ;
    rdfs:label "Part - P543 Part 10 ALiability of executive officers and adverse publicity orders"@en-AU ;
    dct:hasPart C2020A00012:544,
        C2020A00012:545,
        C2020A00012:546,
        C2020A00012:547,
        C2020A00012:548,
        C2020A00012:549 ;
    dct:isPartOf C2020A00012:467 ;
    dct:isReferencedBy C2020A00012: ;
    rdfs:comment "Part 10 ALiability of executive officers and adverse publicity orders - Abrievated Graph Key: P543"@en-AU ;
    skos:broader C2020A00012:544,
        C2020A00012:545,
        C2020A00012:546,
        C2020A00012:547,
        C2020A00012:548,
        C2020A00012:549 ;
    skos:definition "Part 10 ALiability of executive officers and adverse publicity orders"@en-AU ;
    skos:narrower C2020A00012:467 ;
    skos:prefLabel "Part P543"@en-AU ;
    dcat:accessURL <https://www.legislation.gov.au/C2020A00012/2024-07-10/2024-07-10/text/original/epub/OEBPS/document_1/document_1.html#_Toc172119235> ;
    dcat:landingPage "https://www.legislation.gov.au/C2020A00012/2024-07-10/2024-07-10/text/original/epub/OEBPS/document_1/document_1.html#_Toc172119235"^^xsd:anyURI ;
    dcat:theme legcons:Part .

C2020A00012:584 a legcons:Division,
        owl:Class,
        dcat:Resource ;
    rdfs:label "Division - D584 Division 2 Review of decisions"@en-AU ;
    dct:hasPart C2020A00012:585,
        C2020A00012:586,
        C2020A00012:587,
        C2020A00012:588,
        C2020A00012:589,
        C2020A00012:590 ;
    dct:isPartOf C2020A00012:581 ;
    dct:isReferencedBy C2020A00012: ;
    rdfs:comment "Division 2 Review of decisions - Abrievated Graph Key: D584"@en-AU ;
    skos:broader C2020A00012:585,
        C2020A00012:586,
        C2020A00012:587,
        C2020A00012:588,
        C2020A00012:589,
        C2020A00012:590 ;
    skos:definition "Division 2 Review of decisions"@en-AU ;
    skos:narrower C2020A00012:581 ;
    skos:prefLabel "Division D584"@en-AU ;
    dcat:accessURL <https://www.legislation.gov.au/C2020A00012/2024-07-10/2024-07-10/text/original/epub/OEBPS/document_1/document_1.html#_Toc172119276> ;
    dcat:landingPage "https://www.legislation.gov.au/C2020A00012/2024-07-10/2024-07-10/text/original/epub/OEBPS/document_1/document_1.html#_Toc172119276"^^xsd:anyURI ;
    dcat:theme legcons:Division .

C2020A00012:636 a legcons:Division,
        owl:Class,
        dcat:Resource ;
    rdfs:label "Division - D636 Division 2 Taking testing and analysing samples"@en-AU ;
    dct:hasPart C2020A00012:637,
        C2020A00012:638,
        C2020A00012:639,
        C2020A00012:640,
        C2020A00012:641,
        C2020A00012:642 ;
    dct:isPartOf C2020A00012:633 ;
    dct:isReferencedBy C2020A00012: ;
    rdfs:comment "Division 2 Taking testing and analysing samples - Abrievated Graph Key: D636"@en-AU ;
    skos:broader C2020A00012:637,
        C2020A00012:638,
        C2020A00012:639,
        C2020A00012:640,
        C2020A00012:641,
        C2020A00012:642 ;
    skos:definition "Division 2 Taking testing and analysing samples"@en-AU ;
    skos:narrower C2020A00012:633 ;
    skos:prefLabel "Division D636"@en-AU ;
    dcat:accessURL <https://www.legislation.gov.au/C2020A00012/2024-07-10/2024-07-10/text/original/epub/OEBPS/document_1/document_1.html#_Toc172119328> ;
    dcat:landingPage "https://www.legislation.gov.au/C2020A00012/2024-07-10/2024-07-10/text/original/epub/OEBPS/document_1/document_1.html#_Toc172119328"^^xsd:anyURI ;
    dcat:theme legcons:Division .

C2020A00012:149 a legcons:Chapter,
        owl:Class,
        dcat:Resource ;
    rdfs:label "Chapter - C149 Chapter 4 Registered establishments"@en-AU ;
    dct:hasPart C2020A00012:150,
        C2020A00012:152,
        C2020A00012:158,
        C2020A00012:163,
        C2020A00012:171,
        C2020A00012:188,
        C2020A00012:198,
        C2020A00012:204 ;
    dct:isReferencedBy C2020A00012: ;
    rdfs:comment "Chapter 4 Registered establishments - Abrievated Graph Key: C149"@en-AU ;
    skos:broader C2020A00012:150,
        C2020A00012:152,
        C2020A00012:158,
        C2020A00012:163,
        C2020A00012:171,
        C2020A00012:188,
        C2020A00012:198,
        C2020A00012:204 ;
    skos:definition "Chapter 4 Registered establishments"@en-AU ;
    skos:prefLabel "Chapter C149"@en-AU ;
    dcat:accessURL <https://www.legislation.gov.au/C2020A00012/2024-07-10/2024-07-10/text/original/epub/OEBPS/document_1/document_1.html#_Toc172118841> ;
    dcat:landingPage "https://www.legislation.gov.au/C2020A00012/2024-07-10/2024-07-10/text/original/epub/OEBPS/document_1/document_1.html#_Toc172118841"^^xsd:anyURI ;
    dcat:theme legcons:Chapter .

C2020A00012:265 a legcons:Chapter,
        owl:Class,
        dcat:Resource ;
    rdfs:label "Chapter - C265 Chapter 6 Export licences"@en-AU ;
    dct:hasPart C2020A00012:266,
        C2020A00012:268,
        C2020A00012:274,
        C2020A00012:279,
        C2020A00012:286,
        C2020A00012:298,
        C2020A00012:308,
        C2020A00012:312 ;
    dct:isReferencedBy C2020A00012: ;
    rdfs:comment "Chapter 6 Export licences - Abrievated Graph Key: C265"@en-AU ;
    skos:broader C2020A00012:266,
        C2020A00012:268,
        C2020A00012:274,
        C2020A00012:279,
        C2020A00012:286,
        C2020A00012:298,
        C2020A00012:308,
        C2020A00012:312 ;
    skos:definition "Chapter 6 Export licences"@en-AU ;
    skos:prefLabel "Chapter C265"@en-AU ;
    dcat:accessURL <https://www.legislation.gov.au/C2020A00012/2024-07-10/2024-07-10/text/original/epub/OEBPS/document_1/document_1.html#_Toc172118957> ;
    dcat:landingPage "https://www.legislation.gov.au/C2020A00012/2024-07-10/2024-07-10/text/original/epub/OEBPS/document_1/document_1.html#_Toc172118957"^^xsd:anyURI ;
    dcat:theme legcons:Chapter .

C2020A00012:383 a legcons:Division,
        owl:Class,
        dcat:Resource ;
    rdfs:label "Division - D383 Division 2 General"@en-AU ;
    dct:hasPart C2020A00012:384,
        C2020A00012:385,
        C2020A00012:386,
        C2020A00012:387,
        C2020A00012:388,
        C2020A00012:389,
        C2020A00012:390 ;
    dct:isPartOf C2020A00012:380 ;
    dct:isReferencedBy C2020A00012: ;
    rdfs:comment "Division 2 General - Abrievated Graph Key: D383"@en-AU ;
    skos:broader C2020A00012:384,
        C2020A00012:385,
        C2020A00012:386,
        C2020A00012:387,
        C2020A00012:388,
        C2020A00012:389,
        C2020A00012:390 ;
    skos:definition "Division 2 General"@en-AU ;
    skos:narrower C2020A00012:380 ;
    skos:prefLabel "Division D383"@en-AU ;
    dcat:accessURL <https://www.legislation.gov.au/C2020A00012/2024-07-10/2024-07-10/text/original/epub/OEBPS/document_1/document_1.html#_Toc172119075> ;
    dcat:landingPage "https://www.legislation.gov.au/C2020A00012/2024-07-10/2024-07-10/text/original/epub/OEBPS/document_1/document_1.html#_Toc172119075"^^xsd:anyURI ;
    dcat:theme legcons:Division .

C2020A00012:457 a legcons:Division,
        owl:Class,
        dcat:Resource ;
    rdfs:label "Division - D457 Division 3 Offences and civil penalty provisions"@en-AU ;
    dct:hasPart C2020A00012:458,
        C2020A00012:459,
        C2020A00012:460,
        C2020A00012:461,
        C2020A00012:462,
        C2020A00012:463,
        C2020A00012:464 ;
    dct:isPartOf C2020A00012:449 ;
    dct:isReferencedBy C2020A00012: ;
    rdfs:comment "Division 3 Offences and civil penalty provisions - Abrievated Graph Key: D457"@en-AU ;
    skos:broader C2020A00012:458,
        C2020A00012:459,
        C2020A00012:460,
        C2020A00012:461,
        C2020A00012:462,
        C2020A00012:463,
        C2020A00012:464 ;
    skos:definition "Division 3 Offences and civil penalty provisions"@en-AU ;
    skos:narrower C2020A00012:449 ;
    skos:prefLabel "Division D457"@en-AU ;
    dcat:accessURL <https://www.legislation.gov.au/C2020A00012/2024-07-10/2024-07-10/text/original/epub/OEBPS/document_1/document_1.html#_Toc172119149> ;
    dcat:landingPage "https://www.legislation.gov.au/C2020A00012/2024-07-10/2024-07-10/text/original/epub/OEBPS/document_1/document_1.html#_Toc172119149"^^xsd:anyURI ;
    dcat:theme legcons:Division .

C2020A00012:566 a legcons:Chapter,
        owl:Class,
        dcat:Resource ;
    rdfs:label "Chapter - C566 Chapter 11 Miscellaneous"@en-AU ;
    dct:hasPart C2020A00012:567,
        C2020A00012:575,
        C2020A00012:581,
        C2020A00012:591,
        C2020A00012:613,
        C2020A00012:628,
        C2020A00012:633,
        C2020A00012:680 ;
    dct:isReferencedBy C2020A00012: ;
    rdfs:comment "Chapter 11 Miscellaneous - Abrievated Graph Key: C566"@en-AU ;
    skos:broader C2020A00012:567,
        C2020A00012:575,
        C2020A00012:581,
        C2020A00012:591,
        C2020A00012:613,
        C2020A00012:628,
        C2020A00012:633,
        C2020A00012:680 ;
    skos:definition "Chapter 11 Miscellaneous"@en-AU ;
    skos:prefLabel "Chapter C566"@en-AU ;
    dcat:accessURL <https://www.legislation.gov.au/C2020A00012/2024-07-10/2024-07-10/text/original/epub/OEBPS/document_1/document_1.html#_Toc172119258> ;
    dcat:landingPage "https://www.legislation.gov.au/C2020A00012/2024-07-10/2024-07-10/text/original/epub/OEBPS/document_1/document_1.html#_Toc172119258"^^xsd:anyURI ;
    dcat:theme legcons:Chapter .

C2020A00012:662 a legcons:Subdivision,
        owl:Class,
        dcat:Resource ;
    rdfs:label "Subdivision - S662 Subdivision BPrograms"@en-AU ;
    dct:hasPart C2020A00012:663,
        C2020A00012:664,
        C2020A00012:665,
        C2020A00012:666,
        C2020A00012:667,
        C2020A00012:668,
        C2020A00012:669 ;
    dct:isPartOf C2020A00012:656 ;
    dct:isReferencedBy C2020A00012: ;
    rdfs:comment "Subdivision BPrograms - Abrievated Graph Key: S662"@en-AU ;
    skos:broader C2020A00012:663,
        C2020A00012:664,
        C2020A00012:665,
        C2020A00012:666,
        C2020A00012:667,
        C2020A00012:668,
        C2020A00012:669 ;
    skos:definition "Subdivision BPrograms"@en-AU ;
    skos:narrower C2020A00012:656 ;
    skos:prefLabel "Subdivision S662"@en-AU ;
    dcat:accessURL <https://www.legislation.gov.au/C2020A00012/2024-07-10/2024-07-10/text/original/epub/OEBPS/document_1/document_1.html#_Toc172119354> ;
    dcat:landingPage "https://www.legislation.gov.au/C2020A00012/2024-07-10/2024-07-10/text/original/epub/OEBPS/document_1/document_1.html#_Toc172119354"^^xsd:anyURI ;
    dcat:theme legcons:Subdivision .

C2020A00012:27 a legcons:Chapter,
        owl:Class,
        dcat:Resource ;
    rdfs:label "Chapter - C27 Chapter 2 Exporting goods"@en-AU ;
    dct:hasPart C2020A00012:28,
        C2020A00012:66,
        C2020A00012:67,
        C2020A00012:70,
        C2020A00012:79,
        C2020A00012:80,
        C2020A00012:82,
        C2020A00012:86,
        C2020A00012:95 ;
    dct:isReferencedBy C2020A00012: ;
    rdfs:comment "Chapter 2 Exporting goods - Abrievated Graph Key: C27"@en-AU ;
    skos:broader C2020A00012:28,
        C2020A00012:66,
        C2020A00012:67,
        C2020A00012:70,
        C2020A00012:79,
        C2020A00012:80,
        C2020A00012:82,
        C2020A00012:86,
        C2020A00012:95 ;
    skos:definition "Chapter 2 Exporting goods"@en-AU ;
    skos:prefLabel "Chapter C27"@en-AU ;
    dcat:accessURL <https://www.legislation.gov.au/C2020A00012/2024-07-10/2024-07-10/text/original/epub/OEBPS/document_1/document_1.html#_Toc172118719> ;
    dcat:landingPage "https://www.legislation.gov.au/C2020A00012/2024-07-10/2024-07-10/text/original/epub/OEBPS/document_1/document_1.html#_Toc172118719"^^xsd:anyURI ;
    dcat:theme legcons:Chapter .

C2020A00012:633 a legcons:Part,
        owl:Class,
        dcat:Resource ;
    rdfs:label "Part - P633 Part 6 Miscellaneous"@en-AU ;
    dct:hasPart C2020A00012:634,
        C2020A00012:636,
        C2020A00012:643,
        C2020A00012:645,
        C2020A00012:650,
        C2020A00012:654,
        C2020A00012:656,
        C2020A00012:670 ;
    dct:isPartOf C2020A00012:566 ;
    dct:isReferencedBy C2020A00012: ;
    rdfs:comment "Part 6 Miscellaneous - Abrievated Graph Key: P633"@en-AU ;
    skos:broader C2020A00012:634,
        C2020A00012:636,
        C2020A00012:643,
        C2020A00012:645,
        C2020A00012:650,
        C2020A00012:654,
        C2020A00012:656,
        C2020A00012:670 ;
    skos:definition "Part 6 Miscellaneous"@en-AU ;
    skos:narrower C2020A00012:566 ;
    skos:prefLabel "Part P633"@en-AU ;
    dcat:accessURL <https://www.legislation.gov.au/C2020A00012/2024-07-10/2024-07-10/text/original/epub/OEBPS/document_1/document_1.html#_Toc172119325> ;
    dcat:landingPage "https://www.legislation.gov.au/C2020A00012/2024-07-10/2024-07-10/text/original/epub/OEBPS/document_1/document_1.html#_Toc172119325"^^xsd:anyURI ;
    dcat:theme legcons:Part .

C2020A00012:70 a legcons:Division,
        owl:Class,
        dcat:Resource ;
    rdfs:label "Division - D70 Division 2 Exemptions"@en-AU ;
    dct:hasPart C2020A00012:71,
        C2020A00012:72,
        C2020A00012:73,
        C2020A00012:74,
        C2020A00012:75,
        C2020A00012:76,
        C2020A00012:77,
        C2020A00012:78 ;
    dct:isPartOf C2020A00012:27 ;
    dct:isReferencedBy C2020A00012: ;
    rdfs:comment "Division 2 Exemptions - Abrievated Graph Key: D70"@en-AU ;
    skos:broader C2020A00012:71,
        C2020A00012:72,
        C2020A00012:73,
        C2020A00012:74,
        C2020A00012:75,
        C2020A00012:76,
        C2020A00012:77,
        C2020A00012:78 ;
    skos:definition "Division 2 Exemptions"@en-AU ;
    skos:narrower C2020A00012:27 ;
    skos:prefLabel "Division D70"@en-AU ;
    dcat:accessURL <https://www.legislation.gov.au/C2020A00012/2024-07-10/2024-07-10/text/original/epub/OEBPS/document_1/document_1.html#_Toc172118762> ;
    dcat:landingPage "https://www.legislation.gov.au/C2020A00012/2024-07-10/2024-07-10/text/original/epub/OEBPS/document_1/document_1.html#_Toc172118762"^^xsd:anyURI ;
    dcat:theme legcons:Division .

C2020A00012:86 a legcons:Division,
        owl:Class,
        dcat:Resource ;
    rdfs:label "Division - D86 Division 3 Issue of government certificate"@en-AU ;
    dct:hasPart C2020A00012:87,
        C2020A00012:88,
        C2020A00012:89,
        C2020A00012:90,
        C2020A00012:91,
        C2020A00012:92,
        C2020A00012:93,
        C2020A00012:94 ;
    dct:isPartOf C2020A00012:27 ;
    dct:isReferencedBy C2020A00012: ;
    rdfs:comment "Division 3 Issue of government certificate - Abrievated Graph Key: D86"@en-AU ;
    skos:broader C2020A00012:87,
        C2020A00012:88,
        C2020A00012:89,
        C2020A00012:90,
        C2020A00012:91,
        C2020A00012:92,
        C2020A00012:93,
        C2020A00012:94 ;
    skos:definition "Division 3 Issue of government certificate"@en-AU ;
    skos:narrower C2020A00012:27 ;
    skos:prefLabel "Division D86"@en-AU ;
    dcat:accessURL <https://www.legislation.gov.au/C2020A00012/2024-07-10/2024-07-10/text/original/epub/OEBPS/document_1/document_1.html#_Toc172118778> ;
    dcat:landingPage "https://www.legislation.gov.au/C2020A00012/2024-07-10/2024-07-10/text/original/epub/OEBPS/document_1/document_1.html#_Toc172118778"^^xsd:anyURI ;
    dcat:theme legcons:Division .

C2020A00012:670 a legcons:Division,
        owl:Class,
        dcat:Resource ;
    rdfs:label "Division - D670 Division 7 Miscellaneous"@en-AU ;
    dct:hasPart C2020A00012:671,
        C2020A00012:672,
        C2020A00012:673,
        C2020A00012:674,
        C2020A00012:675,
        C2020A00012:676,
        C2020A00012:677,
        C2020A00012:678,
        C2020A00012:679 ;
    dct:isPartOf C2020A00012:633 ;
    dct:isReferencedBy C2020A00012: ;
    rdfs:comment "Division 7 Miscellaneous - Abrievated Graph Key: D670"@en-AU ;
    skos:broader C2020A00012:671,
        C2020A00012:672,
        C2020A00012:673,
        C2020A00012:674,
        C2020A00012:675,
        C2020A00012:676,
        C2020A00012:677,
        C2020A00012:678,
        C2020A00012:679 ;
    skos:definition "Division 7 Miscellaneous"@en-AU ;
    skos:narrower C2020A00012:633 ;
    skos:prefLabel "Division D670"@en-AU ;
    dcat:accessURL <https://www.legislation.gov.au/C2020A00012/2024-07-10/2024-07-10/text/original/epub/OEBPS/document_1/document_1.html#_Toc172119362> ;
    dcat:landingPage "https://www.legislation.gov.au/C2020A00012/2024-07-10/2024-07-10/text/original/epub/OEBPS/document_1/document_1.html#_Toc172119362"^^xsd:anyURI ;
    dcat:theme legcons:Division .

C2020A00012:467 a legcons:Chapter,
        owl:Class,
        dcat:Resource ;
    rdfs:label "Chapter - C467 Chapter 10 Compliance and enforcement"@en-AU ;
    dct:hasPart C2020A00012:468,
        C2020A00012:471,
        C2020A00012:477,
        C2020A00012:483,
        C2020A00012:503,
        C2020A00012:516,
        C2020A00012:522,
        C2020A00012:527,
        C2020A00012:533,
        C2020A00012:538,
        C2020A00012:543,
        C2020A00012:550 ;
    dct:isReferencedBy C2020A00012: ;
    rdfs:comment "Chapter 10 Compliance and enforcement - Abrievated Graph Key: C467"@en-AU ;
    skos:broader C2020A00012:468,
        C2020A00012:471,
        C2020A00012:477,
        C2020A00012:483,
        C2020A00012:503,
        C2020A00012:516,
        C2020A00012:522,
        C2020A00012:527,
        C2020A00012:533,
        C2020A00012:538,
        C2020A00012:543,
        C2020A00012:550 ;
    skos:definition "Chapter 10 Compliance and enforcement"@en-AU ;
    skos:prefLabel "Chapter C467"@en-AU ;
    dcat:accessURL <https://www.legislation.gov.au/C2020A00012/2024-07-10/2024-07-10/text/original/epub/OEBPS/document_1/document_1.html#_Toc172119159> ;
    dcat:landingPage "https://www.legislation.gov.au/C2020A00012/2024-07-10/2024-07-10/text/original/epub/OEBPS/document_1/document_1.html#_Toc172119159"^^xsd:anyURI ;
    dcat:theme legcons:Chapter .

C2020A00012:594 a legcons:Division,
        owl:Class,
        dcat:Resource ;
    rdfs:label "Division - D594 Division 2 Authorised uses and disclosures of relevant information"@en-AU ;
    dct:hasPart C2020A00012:595,
        C2020A00012:596,
        C2020A00012:597,
        C2020A00012:598,
        C2020A00012:599,
        C2020A00012:600,
        C2020A00012:601,
        C2020A00012:602,
        C2020A00012:603,
        C2020A00012:604,
        C2020A00012:605,
        C2020A00012:606,
        C2020A00012:607,
        C2020A00012:608,
        C2020A00012:609 ;
    dct:isPartOf C2020A00012:591 ;
    dct:isReferencedBy C2020A00012: ;
    rdfs:comment "Division 2 Authorised uses and disclosures of relevant information - Abrievated Graph Key: D594"@en-AU ;
    skos:broader C2020A00012:595,
        C2020A00012:596,
        C2020A00012:597,
        C2020A00012:598,
        C2020A00012:599,
        C2020A00012:600,
        C2020A00012:601,
        C2020A00012:602,
        C2020A00012:603,
        C2020A00012:604,
        C2020A00012:605,
        C2020A00012:606,
        C2020A00012:607,
        C2020A00012:608,
        C2020A00012:609 ;
    skos:definition "Division 2 Authorised uses and disclosures of relevant information"@en-AU ;
    skos:narrower C2020A00012:591 ;
    skos:prefLabel "Division D594"@en-AU ;
    dcat:accessURL <https://www.legislation.gov.au/C2020A00012/2024-07-10/2024-07-10/text/original/epub/OEBPS/document_1/document_1.html#_Toc172119286> ;
    dcat:landingPage "https://www.legislation.gov.au/C2020A00012/2024-07-10/2024-07-10/text/original/epub/OEBPS/document_1/document_1.html#_Toc172119286"^^xsd:anyURI ;
    dcat:theme legcons:Division .

C2020A00012:1 a legcons:Chapter,
        owl:Class,
        dcat:Resource ;
    rdfs:label "Chapter - C1 Chapter 1 Preliminary"@en-AU ;
    dct:hasPart C2020A00012:10,
        C2020A00012:11,
        C2020A00012:12,
        C2020A00012:13,
        C2020A00012:14,
        C2020A00012:15,
        C2020A00012:16,
        C2020A00012:17,
        C2020A00012:18,
        C2020A00012:19,
        C2020A00012:2,
        C2020A00012:20,
        C2020A00012:21,
        C2020A00012:22,
        C2020A00012:23,
        C2020A00012:24,
        C2020A00012:25,
        C2020A00012:26,
        C2020A00012:3,
        C2020A00012:4,
        C2020A00012:5,
        C2020A00012:6,
        C2020A00012:7,
        C2020A00012:8,
        C2020A00012:9 ;
    dct:isReferencedBy C2020A00012: ;
    rdfs:comment "Chapter 1 Preliminary - Abrievated Graph Key: C1"@en-AU ;
    skos:broader C2020A00012:10,
        C2020A00012:11,
        C2020A00012:12,
        C2020A00012:13,
        C2020A00012:14,
        C2020A00012:15,
        C2020A00012:16,
        C2020A00012:17,
        C2020A00012:18,
        C2020A00012:19,
        C2020A00012:2,
        C2020A00012:20,
        C2020A00012:21,
        C2020A00012:22,
        C2020A00012:23,
        C2020A00012:24,
        C2020A00012:25,
        C2020A00012:26,
        C2020A00012:3,
        C2020A00012:4,
        C2020A00012:5,
        C2020A00012:6,
        C2020A00012:7,
        C2020A00012:8,
        C2020A00012:9 ;
    skos:definition "Chapter 1 Preliminary"@en-AU ;
    skos:prefLabel "Chapter C1"@en-AU ;
    dcat:accessURL <https://www.legislation.gov.au/C2020A00012/2024-07-10/2024-07-10/text/original/epub/OEBPS/document_1/document_1.html#_Toc172118693> ;
    dcat:landingPage "https://www.legislation.gov.au/C2020A00012/2024-07-10/2024-07-10/text/original/epub/OEBPS/document_1/document_1.html#_Toc172118693"^^xsd:anyURI ;
    dcat:theme legcons:Chapter .

C2020A00012:28 a legcons:Part,
        owl:Class,
        dcat:Resource ;
    rdfs:label "Part - P28 Part 1 Goods and exports"@en-AU ;
    dct:hasPart C2020A00012:29,
        C2020A00012:31,
        C2020A00012:40,
        C2020A00012:41,
        C2020A00012:42,
        C2020A00012:43,
        C2020A00012:44,
        C2020A00012:45,
        C2020A00012:46,
        C2020A00012:47,
        C2020A00012:48,
        C2020A00012:49,
        C2020A00012:50,
        C2020A00012:51,
        C2020A00012:52,
        C2020A00012:53,
        C2020A00012:54,
        C2020A00012:55,
        C2020A00012:56,
        C2020A00012:57,
        C2020A00012:58,
        C2020A00012:59,
        C2020A00012:60,
        C2020A00012:61,
        C2020A00012:62,
        C2020A00012:63,
        C2020A00012:64,
        C2020A00012:65 ;
    dct:isPartOf C2020A00012:27 ;
    dct:isReferencedBy C2020A00012: ;
    rdfs:comment "Part 1 Goods and exports - Abrievated Graph Key: P28"@en-AU ;
    skos:broader C2020A00012:29,
        C2020A00012:31,
        C2020A00012:40,
        C2020A00012:41,
        C2020A00012:42,
        C2020A00012:43,
        C2020A00012:44,
        C2020A00012:45,
        C2020A00012:46,
        C2020A00012:47,
        C2020A00012:48,
        C2020A00012:49,
        C2020A00012:50,
        C2020A00012:51,
        C2020A00012:52,
        C2020A00012:53,
        C2020A00012:54,
        C2020A00012:55,
        C2020A00012:56,
        C2020A00012:57,
        C2020A00012:58,
        C2020A00012:59,
        C2020A00012:60,
        C2020A00012:61,
        C2020A00012:62,
        C2020A00012:63,
        C2020A00012:64,
        C2020A00012:65 ;
    skos:definition "Part 1 Goods and exports"@en-AU ;
    skos:narrower C2020A00012:27 ;
    skos:prefLabel "Part P28"@en-AU ;
    dcat:accessURL <https://www.legislation.gov.au/C2020A00012/2024-07-10/2024-07-10/text/original/epub/OEBPS/document_1/document_1.html#_Toc172118720> ;
    dcat:landingPage "https://www.legislation.gov.au/C2020A00012/2024-07-10/2024-07-10/text/original/epub/OEBPS/document_1/document_1.html#_Toc172118720"^^xsd:anyURI ;
    dcat:theme legcons:Part .

C2020A00012: a owl:Class,
        dcat:Dataset,
        dcat:Resource ;
    rdfs:label "Export Control Act 2020" ;
    dct:Jurisdiction " Department of Agriculture, Fisheries and Forestry "@en-AU ;
    dct:created "2024-08-26T09:36:01.774736"^^xsd:dateTime ;
    dct:creator "https://orcid.org/0009-0007-8434-7325"^^xsd:anyURI ;
    dct:date "2024-07-10T00:00:00+10:00"^^xsd:dateTime ;
    dct:description "Export Control Act 2020"@en-AU ;
    dct:identifier "https://www.legislation.gov.au/C2020A00012/latest"^^xsd:anyURI ;
    dct:license <https://creativecommons.org/licenses/by-sa/4.0/> ;
    dct:source "scheme=AGLSTERMS.AglsAgent; corporateName=Office Parliamentary Counsel; address=Locked Bag 30 Kingston ACT 2604; contact=+61 2 6120 1400"@en-AU ;
    dct:subject "Export Control Act 2020"@en-AU ;
    dct:title "Export Control Act 2020"@en-AU ;
    owl:imports legcons: ;
    dcat:theme legcons:Chapter,
        legcons:Division,
        legcons:Endnotes,
        legcons:Item,
        legcons:Part,
        legcons:Subdivision ;
    schema:identifier "C2020A00012" ;
    schema:status "In force" ;
    schema:version "C2024C00313 (C07)" .

