@prefix C2024A00060: <http://example.org/au/leg/dataset/C2024A00060/> .
@prefix dcat: <http://www.w3.org/ns/dcat#> .
@prefix dct: <http://purl.org/dc/terms/> .
@prefix legcons: <http://example.org/au/leg/concepts/> .
@prefix owl: <http://www.w3.org/2002/07/owl#> .
@prefix rdfs: <http://www.w3.org/2000/01/rdf-schema#> .
@prefix schema: <https://schema.org/> .
@prefix skos: <http://www.w3.org/2004/02/skos/core#> .
@prefix xsd: <http://www.w3.org/2001/XMLSchema#> .

C2024A00060:1 a legcons:Item,
        owl:Class,
        dcat:Resource ;
    rdfs:label "Item - I1 1  Short title"@en-AU ;
    dct:isReferencedBy C2024A00060: ;
    rdfs:comment "1  Short title - Abrievated Graph Key: I1"@en-AU ;
    skos:definition "1  Short title"@en-AU ;
    skos:prefLabel "Item I1"@en-AU ;
    dcat:accessURL <https://www.legislation.gov.au/C2024A00060/asmade/2024-07-09/text/original/epub/OEBPS/document_1/document_1.html#_Toc171517261> ;
    dcat:landingPage "https://www.legislation.gov.au/C2024A00060/asmade/2024-07-09/text/original/epub/OEBPS/document_1/document_1.html#_Toc171517261"^^xsd:anyURI ;
    dcat:theme legcons:Item .

C2024A00060:2 a legcons:Item,
        owl:Class,
        dcat:Resource ;
    rdfs:label "Item - I2 2  Commencement"@en-AU ;
    dct:isReferencedBy C2024A00060: ;
    rdfs:comment "2  Commencement - Abrievated Graph Key: I2"@en-AU ;
    skos:definition "2  Commencement"@en-AU ;
    skos:prefLabel "Item I2"@en-AU ;
    dcat:accessURL <https://www.legislation.gov.au/C2024A00060/asmade/2024-07-09/text/original/epub/OEBPS/document_1/document_1.html#_Toc171517262> ;
    dcat:landingPage "https://www.legislation.gov.au/C2024A00060/asmade/2024-07-09/text/original/epub/OEBPS/document_1/document_1.html#_Toc171517262"^^xsd:anyURI ;
    dcat:theme legcons:Item .

C2024A00060:10 a legcons:Item,
        owl:Class,
        dcat:Resource ;
    rdfs:label "Item - I10 Egg Industry Service Provision Act 2002"@en-AU ;
    dct:isPartOf C2024A00060:3 ;
    dct:isReferencedBy C2024A00060: ;
    rdfs:comment "Egg Industry Service Provision Act 2002 - Abrievated Graph Key: I10"@en-AU ;
    skos:definition "Egg Industry Service Provision Act 2002"@en-AU ;
    skos:narrower C2024A00060:3 ;
    skos:prefLabel "Item I10"@en-AU ;
    dcat:accessURL <https://www.legislation.gov.au/C2024A00060/asmade/2024-07-09/text/original/epub/OEBPS/document_1/document_1.html#_Toc171517270> ;
    dcat:landingPage "https://www.legislation.gov.au/C2024A00060/asmade/2024-07-09/text/original/epub/OEBPS/document_1/document_1.html#_Toc171517270"^^xsd:anyURI ;
    dcat:theme legcons:Item .

C2024A00060:11 a legcons:Item,
        owl:Class,
        dcat:Resource ;
    rdfs:label "Item - I11 Egg Industry Service Provision Transitional and Consequential Provisions Act 2002"@en-AU ;
    dct:isPartOf C2024A00060:3 ;
    dct:isReferencedBy C2024A00060: ;
    rdfs:comment "Egg Industry Service Provision Transitional and Consequential Provisions Act 2002 - Abrievated Graph Key: I11"@en-AU ;
    skos:definition "Egg Industry Service Provision Transitional and Consequential Provisions Act 2002"@en-AU ;
    skos:narrower C2024A00060:3 ;
    skos:prefLabel "Item I11"@en-AU ;
    dcat:accessURL <https://www.legislation.gov.au/C2024A00060/asmade/2024-07-09/text/original/epub/OEBPS/document_1/document_1.html#_Toc171517271> ;
    dcat:landingPage "https://www.legislation.gov.au/C2024A00060/asmade/2024-07-09/text/original/epub/OEBPS/document_1/document_1.html#_Toc171517271"^^xsd:anyURI ;
    dcat:theme legcons:Item .

C2024A00060:12 a legcons:Item,
        owl:Class,
        dcat:Resource ;
    rdfs:label "Item - I12 Forestry Marketing and Research and Development Services Act 2007"@en-AU ;
    dct:isPartOf C2024A00060:3 ;
    dct:isReferencedBy C2024A00060: ;
    rdfs:comment "Forestry Marketing and Research and Development Services Act 2007 - Abrievated Graph Key: I12"@en-AU ;
    skos:definition "Forestry Marketing and Research and Development Services Act 2007"@en-AU ;
    skos:narrower C2024A00060:3 ;
    skos:prefLabel "Item I12"@en-AU ;
    dcat:accessURL <https://www.legislation.gov.au/C2024A00060/asmade/2024-07-09/text/original/epub/OEBPS/document_1/document_1.html#_Toc171517272> ;
    dcat:landingPage "https://www.legislation.gov.au/C2024A00060/asmade/2024-07-09/text/original/epub/OEBPS/document_1/document_1.html#_Toc171517272"^^xsd:anyURI ;
    dcat:theme legcons:Item .

C2024A00060:13 a legcons:Item,
        owl:Class,
        dcat:Resource ;
    rdfs:label "Item - I13 Horse Disease Response Levy Act 2011"@en-AU ;
    dct:isPartOf C2024A00060:3 ;
    dct:isReferencedBy C2024A00060: ;
    rdfs:comment "Horse Disease Response Levy Act 2011 - Abrievated Graph Key: I13"@en-AU ;
    skos:definition "Horse Disease Response Levy Act 2011"@en-AU ;
    skos:narrower C2024A00060:3 ;
    skos:prefLabel "Item I13"@en-AU ;
    dcat:accessURL <https://www.legislation.gov.au/C2024A00060/asmade/2024-07-09/text/original/epub/OEBPS/document_1/document_1.html#_Toc171517273> ;
    dcat:landingPage "https://www.legislation.gov.au/C2024A00060/asmade/2024-07-09/text/original/epub/OEBPS/document_1/document_1.html#_Toc171517273"^^xsd:anyURI ;
    dcat:theme legcons:Item .

C2024A00060:14 a legcons:Item,
        owl:Class,
        dcat:Resource ;
    rdfs:label "Item - I14 Horse Disease Response Levy Collection Act 2011"@en-AU ;
    dct:isPartOf C2024A00060:3 ;
    dct:isReferencedBy C2024A00060: ;
    rdfs:comment "Horse Disease Response Levy Collection Act 2011 - Abrievated Graph Key: I14"@en-AU ;
    skos:definition "Horse Disease Response Levy Collection Act 2011"@en-AU ;
    skos:narrower C2024A00060:3 ;
    skos:prefLabel "Item I14"@en-AU ;
    dcat:accessURL <https://www.legislation.gov.au/C2024A00060/asmade/2024-07-09/text/original/epub/OEBPS/document_1/document_1.html#_Toc171517274> ;
    dcat:landingPage "https://www.legislation.gov.au/C2024A00060/asmade/2024-07-09/text/original/epub/OEBPS/document_1/document_1.html#_Toc171517274"^^xsd:anyURI ;
    dcat:theme legcons:Item .

C2024A00060:15 a legcons:Item,
        owl:Class,
        dcat:Resource ;
    rdfs:label "Item - I15 Horticulture Marketing and Research and Development Services Act 2000"@en-AU ;
    dct:isPartOf C2024A00060:3 ;
    dct:isReferencedBy C2024A00060: ;
    rdfs:comment "Horticulture Marketing and Research and Development Services Act 2000 - Abrievated Graph Key: I15"@en-AU ;
    skos:definition "Horticulture Marketing and Research and Development Services Act 2000"@en-AU ;
    skos:narrower C2024A00060:3 ;
    skos:prefLabel "Item I15"@en-AU ;
    dcat:accessURL <https://www.legislation.gov.au/C2024A00060/asmade/2024-07-09/text/original/epub/OEBPS/document_1/document_1.html#_Toc171517275> ;
    dcat:landingPage "https://www.legislation.gov.au/C2024A00060/asmade/2024-07-09/text/original/epub/OEBPS/document_1/document_1.html#_Toc171517275"^^xsd:anyURI ;
    dcat:theme legcons:Item .

C2024A00060:16 a legcons:Item,
        owl:Class,
        dcat:Resource ;
    rdfs:label "Item - I16 National Cattle Disease Eradication Account Act 1991"@en-AU ;
    dct:isPartOf C2024A00060:3 ;
    dct:isReferencedBy C2024A00060: ;
    rdfs:comment "National Cattle Disease Eradication Account Act 1991 - Abrievated Graph Key: I16"@en-AU ;
    skos:definition "National Cattle Disease Eradication Account Act 1991"@en-AU ;
    skos:narrower C2024A00060:3 ;
    skos:prefLabel "Item I16"@en-AU ;
    dcat:accessURL <https://www.legislation.gov.au/C2024A00060/asmade/2024-07-09/text/original/epub/OEBPS/document_1/document_1.html#_Toc171517276> ;
    dcat:landingPage "https://www.legislation.gov.au/C2024A00060/asmade/2024-07-09/text/original/epub/OEBPS/document_1/document_1.html#_Toc171517276"^^xsd:anyURI ;
    dcat:theme legcons:Item .

C2024A00060:17 a legcons:Item,
        owl:Class,
        dcat:Resource ;
    rdfs:label "Item - I17 National Residue Survey Administration Act 1992"@en-AU ;
    dct:isPartOf C2024A00060:3 ;
    dct:isReferencedBy C2024A00060: ;
    rdfs:comment "National Residue Survey Administration Act 1992 - Abrievated Graph Key: I17"@en-AU ;
    skos:definition "National Residue Survey Administration Act 1992"@en-AU ;
    skos:narrower C2024A00060:3 ;
    skos:prefLabel "Item I17"@en-AU ;
    dcat:accessURL <https://www.legislation.gov.au/C2024A00060/asmade/2024-07-09/text/original/epub/OEBPS/document_1/document_1.html#_Toc171517277> ;
    dcat:landingPage "https://www.legislation.gov.au/C2024A00060/asmade/2024-07-09/text/original/epub/OEBPS/document_1/document_1.html#_Toc171517277"^^xsd:anyURI ;
    dcat:theme legcons:Item .

C2024A00060:18 a legcons:Item,
        owl:Class,
        dcat:Resource ;
    rdfs:label "Item - I18 National Residue Survey Consequential Provisions Act 1992"@en-AU ;
    dct:isPartOf C2024A00060:3 ;
    dct:isReferencedBy C2024A00060: ;
    rdfs:comment "National Residue Survey Consequential Provisions Act 1992 - Abrievated Graph Key: I18"@en-AU ;
    skos:definition "National Residue Survey Consequential Provisions Act 1992"@en-AU ;
    skos:narrower C2024A00060:3 ;
    skos:prefLabel "Item I18"@en-AU ;
    dcat:accessURL <https://www.legislation.gov.au/C2024A00060/asmade/2024-07-09/text/original/epub/OEBPS/document_1/document_1.html#_Toc171517278> ;
    dcat:landingPage "https://www.legislation.gov.au/C2024A00060/asmade/2024-07-09/text/original/epub/OEBPS/document_1/document_1.html#_Toc171517278"^^xsd:anyURI ;
    dcat:theme legcons:Item .

C2024A00060:19 a legcons:Item,
        owl:Class,
        dcat:Resource ;
    rdfs:label "Item - I19 National Residue Survey Customs Levy Act 1998"@en-AU ;
    dct:isPartOf C2024A00060:3 ;
    dct:isReferencedBy C2024A00060: ;
    rdfs:comment "National Residue Survey Customs Levy Act 1998 - Abrievated Graph Key: I19"@en-AU ;
    skos:definition "National Residue Survey Customs Levy Act 1998"@en-AU ;
    skos:narrower C2024A00060:3 ;
    skos:prefLabel "Item I19"@en-AU ;
    dcat:accessURL <https://www.legislation.gov.au/C2024A00060/asmade/2024-07-09/text/original/epub/OEBPS/document_1/document_1.html#_Toc171517279> ;
    dcat:landingPage "https://www.legislation.gov.au/C2024A00060/asmade/2024-07-09/text/original/epub/OEBPS/document_1/document_1.html#_Toc171517279"^^xsd:anyURI ;
    dcat:theme legcons:Item .

C2024A00060:20 a legcons:Item,
        owl:Class,
        dcat:Resource ;
    rdfs:label "Item - I20 National Residue Survey Excise Levy Act 1998"@en-AU ;
    dct:isPartOf C2024A00060:3 ;
    dct:isReferencedBy C2024A00060: ;
    rdfs:comment "National Residue Survey Excise Levy Act 1998 - Abrievated Graph Key: I20"@en-AU ;
    skos:definition "National Residue Survey Excise Levy Act 1998"@en-AU ;
    skos:narrower C2024A00060:3 ;
    skos:prefLabel "Item I20"@en-AU ;
    dcat:accessURL <https://www.legislation.gov.au/C2024A00060/asmade/2024-07-09/text/original/epub/OEBPS/document_1/document_1.html#_Toc171517280> ;
    dcat:landingPage "https://www.legislation.gov.au/C2024A00060/asmade/2024-07-09/text/original/epub/OEBPS/document_1/document_1.html#_Toc171517280"^^xsd:anyURI ;
    dcat:theme legcons:Item .

C2024A00060:21 a legcons:Item,
        owl:Class,
        dcat:Resource ;
    rdfs:label "Item - I21 National Residue Survey Levies Regulations Validation and Commencement of Amendments Act 1999"@en-AU ;
    dct:isPartOf C2024A00060:3 ;
    dct:isReferencedBy C2024A00060: ;
    rdfs:comment "National Residue Survey Levies Regulations Validation and Commencement of Amendments Act 1999 - Abrievated Graph Key: I21"@en-AU ;
    skos:definition "National Residue Survey Levies Regulations Validation and Commencement of Amendments Act 1999"@en-AU ;
    skos:narrower C2024A00060:3 ;
    skos:prefLabel "Item I21"@en-AU ;
    dcat:accessURL <https://www.legislation.gov.au/C2024A00060/asmade/2024-07-09/text/original/epub/OEBPS/document_1/document_1.html#_Toc171517281> ;
    dcat:landingPage "https://www.legislation.gov.au/C2024A00060/asmade/2024-07-09/text/original/epub/OEBPS/document_1/document_1.html#_Toc171517281"^^xsd:anyURI ;
    dcat:theme legcons:Item .

C2024A00060:22 a legcons:Item,
        owl:Class,
        dcat:Resource ;
    rdfs:label "Item - I22 Pig Industry Transitional Provisions Act 1986"@en-AU ;
    dct:isPartOf C2024A00060:3 ;
    dct:isReferencedBy C2024A00060: ;
    rdfs:comment "Pig Industry Transitional Provisions Act 1986 - Abrievated Graph Key: I22"@en-AU ;
    skos:definition "Pig Industry Transitional Provisions Act 1986"@en-AU ;
    skos:narrower C2024A00060:3 ;
    skos:prefLabel "Item I22"@en-AU ;
    dcat:accessURL <https://www.legislation.gov.au/C2024A00060/asmade/2024-07-09/text/original/epub/OEBPS/document_1/document_1.html#_Toc171517282> ;
    dcat:landingPage "https://www.legislation.gov.au/C2024A00060/asmade/2024-07-09/text/original/epub/OEBPS/document_1/document_1.html#_Toc171517282"^^xsd:anyURI ;
    dcat:theme legcons:Item .

C2024A00060:23 a legcons:Item,
        owl:Class,
        dcat:Resource ;
    rdfs:label "Item - I23 Plant Health Australia Plant Industries Funding Act 2002"@en-AU ;
    dct:isPartOf C2024A00060:3 ;
    dct:isReferencedBy C2024A00060: ;
    rdfs:comment "Plant Health Australia Plant Industries Funding Act 2002 - Abrievated Graph Key: I23"@en-AU ;
    skos:definition "Plant Health Australia Plant Industries Funding Act 2002"@en-AU ;
    skos:narrower C2024A00060:3 ;
    skos:prefLabel "Item I23"@en-AU ;
    dcat:accessURL <https://www.legislation.gov.au/C2024A00060/asmade/2024-07-09/text/original/epub/OEBPS/document_1/document_1.html#_Toc171517283> ;
    dcat:landingPage "https://www.legislation.gov.au/C2024A00060/asmade/2024-07-09/text/original/epub/OEBPS/document_1/document_1.html#_Toc171517283"^^xsd:anyURI ;
    dcat:theme legcons:Item .

C2024A00060:24 a legcons:Item,
        owl:Class,
        dcat:Resource ;
    rdfs:label "Item - I24 Primary Industries Customs Charges Act 1999"@en-AU ;
    dct:isPartOf C2024A00060:3 ;
    dct:isReferencedBy C2024A00060: ;
    rdfs:comment "Primary Industries Customs Charges Act 1999 - Abrievated Graph Key: I24"@en-AU ;
    skos:definition "Primary Industries Customs Charges Act 1999"@en-AU ;
    skos:narrower C2024A00060:3 ;
    skos:prefLabel "Item I24"@en-AU ;
    dcat:accessURL <https://www.legislation.gov.au/C2024A00060/asmade/2024-07-09/text/original/epub/OEBPS/document_1/document_1.html#_Toc171517284> ;
    dcat:landingPage "https://www.legislation.gov.au/C2024A00060/asmade/2024-07-09/text/original/epub/OEBPS/document_1/document_1.html#_Toc171517284"^^xsd:anyURI ;
    dcat:theme legcons:Item .

C2024A00060:25 a legcons:Item,
        owl:Class,
        dcat:Resource ;
    rdfs:label "Item - I25 Primary Industries Excise Levies Act 1999"@en-AU ;
    dct:isPartOf C2024A00060:3 ;
    dct:isReferencedBy C2024A00060: ;
    rdfs:comment "Primary Industries Excise Levies Act 1999 - Abrievated Graph Key: I25"@en-AU ;
    skos:definition "Primary Industries Excise Levies Act 1999"@en-AU ;
    skos:narrower C2024A00060:3 ;
    skos:prefLabel "Item I25"@en-AU ;
    dcat:accessURL <https://www.legislation.gov.au/C2024A00060/asmade/2024-07-09/text/original/epub/OEBPS/document_1/document_1.html#_Toc171517285> ;
    dcat:landingPage "https://www.legislation.gov.au/C2024A00060/asmade/2024-07-09/text/original/epub/OEBPS/document_1/document_1.html#_Toc171517285"^^xsd:anyURI ;
    dcat:theme legcons:Item .

C2024A00060:26 a legcons:Item,
        owl:Class,
        dcat:Resource ;
    rdfs:label "Item - I26 Primary Industries Levies and Charges Collection Act 1991"@en-AU ;
    dct:isPartOf C2024A00060:3 ;
    dct:isReferencedBy C2024A00060: ;
    rdfs:comment "Primary Industries Levies and Charges Collection Act 1991 - Abrievated Graph Key: I26"@en-AU ;
    skos:definition "Primary Industries Levies and Charges Collection Act 1991"@en-AU ;
    skos:narrower C2024A00060:3 ;
    skos:prefLabel "Item I26"@en-AU ;
    dcat:accessURL <https://www.legislation.gov.au/C2024A00060/asmade/2024-07-09/text/original/epub/OEBPS/document_1/document_1.html#_Toc171517286> ;
    dcat:landingPage "https://www.legislation.gov.au/C2024A00060/asmade/2024-07-09/text/original/epub/OEBPS/document_1/document_1.html#_Toc171517286"^^xsd:anyURI ;
    dcat:theme legcons:Item .

C2024A00060:27 a legcons:Item,
        owl:Class,
        dcat:Resource ;
    rdfs:label "Item - I27 Sugar Research and Development Services Act 2013"@en-AU ;
    dct:isPartOf C2024A00060:3 ;
    dct:isReferencedBy C2024A00060: ;
    rdfs:comment "Sugar Research and Development Services Act 2013 - Abrievated Graph Key: I27"@en-AU ;
    skos:definition "Sugar Research and Development Services Act 2013"@en-AU ;
    skos:narrower C2024A00060:3 ;
    skos:prefLabel "Item I27"@en-AU ;
    dcat:accessURL <https://www.legislation.gov.au/C2024A00060/asmade/2024-07-09/text/original/epub/OEBPS/document_1/document_1.html#_Toc171517287> ;
    dcat:landingPage "https://www.legislation.gov.au/C2024A00060/asmade/2024-07-09/text/original/epub/OEBPS/document_1/document_1.html#_Toc171517287"^^xsd:anyURI ;
    dcat:theme legcons:Item .

C2024A00060:28 a legcons:Schedule,
        owl:Class,
        dcat:Resource ;
    rdfs:label "Schedule - S28 Schedule 2 Consequential amendments"@en-AU ;
    dct:isPartOf C2024A00060:3 ;
    dct:isReferencedBy C2024A00060: ;
    rdfs:comment "Schedule 2 Consequential amendments - Abrievated Graph Key: S28"@en-AU ;
    skos:definition "Schedule 2 Consequential amendments"@en-AU ;
    skos:narrower C2024A00060:3 ;
    skos:prefLabel "Schedule S28"@en-AU ;
    dcat:accessURL <https://www.legislation.gov.au/C2024A00060/asmade/2024-07-09/text/original/epub/OEBPS/document_1/document_1.html#_Toc171517288> ;
    dcat:landingPage "https://www.legislation.gov.au/C2024A00060/asmade/2024-07-09/text/original/epub/OEBPS/document_1/document_1.html#_Toc171517288"^^xsd:anyURI ;
    dcat:theme legcons:Schedule .

C2024A00060:29 a legcons:Part,
        owl:Class,
        dcat:Resource ;
    rdfs:label "Part - P29 Part 1 Main amendments"@en-AU ;
    dct:isPartOf C2024A00060:3 ;
    dct:isReferencedBy C2024A00060: ;
    rdfs:comment "Part 1 Main amendments - Abrievated Graph Key: P29"@en-AU ;
    skos:definition "Part 1 Main amendments"@en-AU ;
    skos:narrower C2024A00060:3 ;
    skos:prefLabel "Part P29"@en-AU ;
    dcat:accessURL <https://www.legislation.gov.au/C2024A00060/asmade/2024-07-09/text/original/epub/OEBPS/document_1/document_1.html#_Toc171517289> ;
    dcat:landingPage "https://www.legislation.gov.au/C2024A00060/asmade/2024-07-09/text/original/epub/OEBPS/document_1/document_1.html#_Toc171517289"^^xsd:anyURI ;
    dcat:theme legcons:Part .

C2024A00060:30 a legcons:Item,
        owl:Class,
        dcat:Resource ;
    rdfs:label "Item - I30 Biosecurity Act 2015"@en-AU ;
    dct:isPartOf C2024A00060:3 ;
    dct:isReferencedBy C2024A00060: ;
    rdfs:comment "Biosecurity Act 2015 - Abrievated Graph Key: I30"@en-AU ;
    skos:definition "Biosecurity Act 2015"@en-AU ;
    skos:narrower C2024A00060:3 ;
    skos:prefLabel "Item I30"@en-AU ;
    dcat:accessURL <https://www.legislation.gov.au/C2024A00060/asmade/2024-07-09/text/original/epub/OEBPS/document_1/document_1.html#_Toc171517290> ;
    dcat:landingPage "https://www.legislation.gov.au/C2024A00060/asmade/2024-07-09/text/original/epub/OEBPS/document_1/document_1.html#_Toc171517290"^^xsd:anyURI ;
    dcat:theme legcons:Item .

C2024A00060:31 a legcons:Item,
        owl:Class,
        dcat:Resource ;
    rdfs:label "Item - I31 Fisheries Administration Act 1991"@en-AU ;
    dct:isPartOf C2024A00060:3 ;
    dct:isReferencedBy C2024A00060: ;
    rdfs:comment "Fisheries Administration Act 1991 - Abrievated Graph Key: I31"@en-AU ;
    skos:definition "Fisheries Administration Act 1991"@en-AU ;
    skos:narrower C2024A00060:3 ;
    skos:prefLabel "Item I31"@en-AU ;
    dcat:accessURL <https://www.legislation.gov.au/C2024A00060/asmade/2024-07-09/text/original/epub/OEBPS/document_1/document_1.html#_Toc171517291> ;
    dcat:landingPage "https://www.legislation.gov.au/C2024A00060/asmade/2024-07-09/text/original/epub/OEBPS/document_1/document_1.html#_Toc171517291"^^xsd:anyURI ;
    dcat:theme legcons:Item .

C2024A00060:32 a legcons:Item,
        owl:Class,
        dcat:Resource ;
    rdfs:label "Item - I32 Freedom of Information Act 1982"@en-AU ;
    dct:isPartOf C2024A00060:3 ;
    dct:isReferencedBy C2024A00060: ;
    rdfs:comment "Freedom of Information Act 1982 - Abrievated Graph Key: I32"@en-AU ;
    skos:definition "Freedom of Information Act 1982"@en-AU ;
    skos:narrower C2024A00060:3 ;
    skos:prefLabel "Item I32"@en-AU ;
    dcat:accessURL <https://www.legislation.gov.au/C2024A00060/asmade/2024-07-09/text/original/epub/OEBPS/document_1/document_1.html#_Toc171517292> ;
    dcat:landingPage "https://www.legislation.gov.au/C2024A00060/asmade/2024-07-09/text/original/epub/OEBPS/document_1/document_1.html#_Toc171517292"^^xsd:anyURI ;
    dcat:theme legcons:Item .

C2024A00060:33 a legcons:Item,
        owl:Class,
        dcat:Resource ;
    rdfs:label "Item - I33 Horticulture Marketing and Research and Development Services Repeals and Consequential Provisions Act 2000"@en-AU ;
    dct:isPartOf C2024A00060:3 ;
    dct:isReferencedBy C2024A00060: ;
    rdfs:comment "Horticulture Marketing and Research and Development Services Repeals and Consequential Provisions Act 2000 - Abrievated Graph Key: I33"@en-AU ;
    skos:definition "Horticulture Marketing and Research and Development Services Repeals and Consequential Provisions Act 2000"@en-AU ;
    skos:narrower C2024A00060:3 ;
    skos:prefLabel "Item I33"@en-AU ;
    dcat:accessURL <https://www.legislation.gov.au/C2024A00060/asmade/2024-07-09/text/original/epub/OEBPS/document_1/document_1.html#_Toc171517293> ;
    dcat:landingPage "https://www.legislation.gov.au/C2024A00060/asmade/2024-07-09/text/original/epub/OEBPS/document_1/document_1.html#_Toc171517293"^^xsd:anyURI ;
    dcat:theme legcons:Item .

C2024A00060:34 a legcons:Item,
        owl:Class,
        dcat:Resource ;
    rdfs:label "Item - I34 Natural Heritage Trust of Australia Act 1997"@en-AU ;
    dct:isPartOf C2024A00060:3 ;
    dct:isReferencedBy C2024A00060: ;
    rdfs:comment "Natural Heritage Trust of Australia Act 1997 - Abrievated Graph Key: I34"@en-AU ;
    skos:definition "Natural Heritage Trust of Australia Act 1997"@en-AU ;
    skos:narrower C2024A00060:3 ;
    skos:prefLabel "Item I34"@en-AU ;
    dcat:accessURL <https://www.legislation.gov.au/C2024A00060/asmade/2024-07-09/text/original/epub/OEBPS/document_1/document_1.html#_Toc171517294> ;
    dcat:landingPage "https://www.legislation.gov.au/C2024A00060/asmade/2024-07-09/text/original/epub/OEBPS/document_1/document_1.html#_Toc171517294"^^xsd:anyURI ;
    dcat:theme legcons:Item .

C2024A00060:35 a legcons:Item,
        owl:Class,
        dcat:Resource ;
    rdfs:label "Item - I35 Pig Industry Act 2001"@en-AU ;
    dct:isPartOf C2024A00060:3 ;
    dct:isReferencedBy C2024A00060: ;
    rdfs:comment "Pig Industry Act 2001 - Abrievated Graph Key: I35"@en-AU ;
    skos:definition "Pig Industry Act 2001"@en-AU ;
    skos:narrower C2024A00060:3 ;
    skos:prefLabel "Item I35"@en-AU ;
    dcat:accessURL <https://www.legislation.gov.au/C2024A00060/asmade/2024-07-09/text/original/epub/OEBPS/document_1/document_1.html#_Toc171517295> ;
    dcat:landingPage "https://www.legislation.gov.au/C2024A00060/asmade/2024-07-09/text/original/epub/OEBPS/document_1/document_1.html#_Toc171517295"^^xsd:anyURI ;
    dcat:theme legcons:Item .

C2024A00060:36 a legcons:Item,
        owl:Class,
        dcat:Resource ;
    rdfs:label "Item - I36 Primary Industries Research and Development Act 1989"@en-AU ;
    dct:isPartOf C2024A00060:3 ;
    dct:isReferencedBy C2024A00060: ;
    rdfs:comment "Primary Industries Research and Development Act 1989 - Abrievated Graph Key: I36"@en-AU ;
    skos:definition "Primary Industries Research and Development Act 1989"@en-AU ;
    skos:narrower C2024A00060:3 ;
    skos:prefLabel "Item I36"@en-AU ;
    dcat:accessURL <https://www.legislation.gov.au/C2024A00060/asmade/2024-07-09/text/original/epub/OEBPS/document_1/document_1.html#_Toc171517296> ;
    dcat:landingPage "https://www.legislation.gov.au/C2024A00060/asmade/2024-07-09/text/original/epub/OEBPS/document_1/document_1.html#_Toc171517296"^^xsd:anyURI ;
    dcat:theme legcons:Item .

C2024A00060:37 a legcons:Item,
        owl:Class,
        dcat:Resource ;
    rdfs:label "Item - I37 Renewable Energy Electricity Act 2000"@en-AU ;
    dct:isPartOf C2024A00060:3 ;
    dct:isReferencedBy C2024A00060: ;
    rdfs:comment "Renewable Energy Electricity Act 2000 - Abrievated Graph Key: I37"@en-AU ;
    skos:definition "Renewable Energy Electricity Act 2000"@en-AU ;
    skos:narrower C2024A00060:3 ;
    skos:prefLabel "Item I37"@en-AU ;
    dcat:accessURL <https://www.legislation.gov.au/C2024A00060/asmade/2024-07-09/text/original/epub/OEBPS/document_1/document_1.html#_Toc171517303> ;
    dcat:landingPage "https://www.legislation.gov.au/C2024A00060/asmade/2024-07-09/text/original/epub/OEBPS/document_1/document_1.html#_Toc171517303"^^xsd:anyURI ;
    dcat:theme legcons:Item .

C2024A00060:38 a legcons:Item,
        owl:Class,
        dcat:Resource ;
    rdfs:label "Item - I38 Sugar Research and Development Services Consequential Amendments and Transitional Provisions Act 2013"@en-AU ;
    dct:isPartOf C2024A00060:3 ;
    dct:isReferencedBy C2024A00060: ;
    rdfs:comment "Sugar Research and Development Services Consequential Amendments and Transitional Provisions Act 2013 - Abrievated Graph Key: I38"@en-AU ;
    skos:definition "Sugar Research and Development Services Consequential Amendments and Transitional Provisions Act 2013"@en-AU ;
    skos:narrower C2024A00060:3 ;
    skos:prefLabel "Item I38"@en-AU ;
    dcat:accessURL <https://www.legislation.gov.au/C2024A00060/asmade/2024-07-09/text/original/epub/OEBPS/document_1/document_1.html#_Toc171517304> ;
    dcat:landingPage "https://www.legislation.gov.au/C2024A00060/asmade/2024-07-09/text/original/epub/OEBPS/document_1/document_1.html#_Toc171517304"^^xsd:anyURI ;
    dcat:theme legcons:Item .

C2024A00060:39 a legcons:Item,
        owl:Class,
        dcat:Resource ;
    rdfs:label "Item - I39 Wine Australia Act 2013"@en-AU ;
    dct:isPartOf C2024A00060:3 ;
    dct:isReferencedBy C2024A00060: ;
    rdfs:comment "Wine Australia Act 2013 - Abrievated Graph Key: I39"@en-AU ;
    skos:definition "Wine Australia Act 2013"@en-AU ;
    skos:narrower C2024A00060:3 ;
    skos:prefLabel "Item I39"@en-AU ;
    dcat:accessURL <https://www.legislation.gov.au/C2024A00060/asmade/2024-07-09/text/original/epub/OEBPS/document_1/document_1.html#_Toc171517305> ;
    dcat:landingPage "https://www.legislation.gov.au/C2024A00060/asmade/2024-07-09/text/original/epub/OEBPS/document_1/document_1.html#_Toc171517305"^^xsd:anyURI ;
    dcat:theme legcons:Item .

C2024A00060:4 a legcons:Schedule,
        owl:Class,
        dcat:Resource ;
    rdfs:label "Schedule - S4 Schedule 1 Repeals"@en-AU ;
    dct:isPartOf C2024A00060:3 ;
    dct:isReferencedBy C2024A00060: ;
    rdfs:comment "Schedule 1 Repeals - Abrievated Graph Key: S4"@en-AU ;
    skos:definition "Schedule 1 Repeals"@en-AU ;
    skos:narrower C2024A00060:3 ;
    skos:prefLabel "Schedule S4"@en-AU ;
    dcat:accessURL <https://www.legislation.gov.au/C2024A00060/asmade/2024-07-09/text/original/epub/OEBPS/document_1/document_1.html#_Toc171517264> ;
    dcat:landingPage "https://www.legislation.gov.au/C2024A00060/asmade/2024-07-09/text/original/epub/OEBPS/document_1/document_1.html#_Toc171517264"^^xsd:anyURI ;
    dcat:theme legcons:Schedule .

C2024A00060:40 a legcons:Item,
        owl:Class,
        dcat:Resource ;
    rdfs:label "Item - I40 Wool Services Privatisation Act 2000"@en-AU ;
    dct:isPartOf C2024A00060:3 ;
    dct:isReferencedBy C2024A00060: ;
    rdfs:comment "Wool Services Privatisation Act 2000 - Abrievated Graph Key: I40"@en-AU ;
    skos:definition "Wool Services Privatisation Act 2000"@en-AU ;
    skos:narrower C2024A00060:3 ;
    skos:prefLabel "Item I40"@en-AU ;
    dcat:accessURL <https://www.legislation.gov.au/C2024A00060/asmade/2024-07-09/text/original/epub/OEBPS/document_1/document_1.html#_Toc171517308> ;
    dcat:landingPage "https://www.legislation.gov.au/C2024A00060/asmade/2024-07-09/text/original/epub/OEBPS/document_1/document_1.html#_Toc171517308"^^xsd:anyURI ;
    dcat:theme legcons:Item .

C2024A00060:41 a legcons:Part,
        owl:Class,
        dcat:Resource ;
    rdfs:label "Part - P41 Part 2 Other amendments"@en-AU ;
    dct:isPartOf C2024A00060:3 ;
    dct:isReferencedBy C2024A00060: ;
    rdfs:comment "Part 2 Other amendments - Abrievated Graph Key: P41"@en-AU ;
    skos:definition "Part 2 Other amendments"@en-AU ;
    skos:narrower C2024A00060:3 ;
    skos:prefLabel "Part P41"@en-AU ;
    dcat:accessURL <https://www.legislation.gov.au/C2024A00060/asmade/2024-07-09/text/original/epub/OEBPS/document_1/document_1.html#_Toc171517309> ;
    dcat:landingPage "https://www.legislation.gov.au/C2024A00060/asmade/2024-07-09/text/original/epub/OEBPS/document_1/document_1.html#_Toc171517309"^^xsd:anyURI ;
    dcat:theme legcons:Part .

C2024A00060:42 a legcons:Item,
        owl:Class,
        dcat:Resource ;
    rdfs:label "Item - I42 Export Control Act 2020"@en-AU ;
    dct:isPartOf C2024A00060:3 ;
    dct:isReferencedBy C2024A00060: ;
    rdfs:comment "Export Control Act 2020 - Abrievated Graph Key: I42"@en-AU ;
    skos:definition "Export Control Act 2020"@en-AU ;
    skos:narrower C2024A00060:3 ;
    skos:prefLabel "Item I42"@en-AU ;
    dcat:accessURL <https://www.legislation.gov.au/C2024A00060/asmade/2024-07-09/text/original/epub/OEBPS/document_1/document_1.html#_Toc171517310> ;
    dcat:landingPage "https://www.legislation.gov.au/C2024A00060/asmade/2024-07-09/text/original/epub/OEBPS/document_1/document_1.html#_Toc171517310"^^xsd:anyURI ;
    dcat:theme legcons:Item .

C2024A00060:43 a legcons:Item,
        owl:Class,
        dcat:Resource ;
    rdfs:label "Item - I43 Inspector General of Live Animal Exports Act 2019"@en-AU ;
    dct:isPartOf C2024A00060:3 ;
    dct:isReferencedBy C2024A00060: ;
    rdfs:comment "Inspector General of Live Animal Exports Act 2019 - Abrievated Graph Key: I43"@en-AU ;
    skos:definition "Inspector General of Live Animal Exports Act 2019"@en-AU ;
    skos:narrower C2024A00060:3 ;
    skos:prefLabel "Item I43"@en-AU ;
    dcat:accessURL <https://www.legislation.gov.au/C2024A00060/asmade/2024-07-09/text/original/epub/OEBPS/document_1/document_1.html#_Toc171517311> ;
    dcat:landingPage "https://www.legislation.gov.au/C2024A00060/asmade/2024-07-09/text/original/epub/OEBPS/document_1/document_1.html#_Toc171517311"^^xsd:anyURI ;
    dcat:theme legcons:Item .

C2024A00060:44 a legcons:Schedule,
        owl:Class,
        dcat:Resource ;
    rdfs:label "Schedule - S44 Schedule 3 Application and transitional provisionsoperation of new law"@en-AU ;
    dct:isPartOf C2024A00060:3 ;
    dct:isReferencedBy C2024A00060: ;
    rdfs:comment "Schedule 3 Application and transitional provisionsoperation of new law - Abrievated Graph Key: S44"@en-AU ;
    skos:definition "Schedule 3 Application and transitional provisionsoperation of new law"@en-AU ;
    skos:narrower C2024A00060:3 ;
    skos:prefLabel "Schedule S44"@en-AU ;
    dcat:accessURL <https://www.legislation.gov.au/C2024A00060/asmade/2024-07-09/text/original/epub/OEBPS/document_1/document_1.html#_Toc171517312> ;
    dcat:landingPage "https://www.legislation.gov.au/C2024A00060/asmade/2024-07-09/text/original/epub/OEBPS/document_1/document_1.html#_Toc171517312"^^xsd:anyURI ;
    dcat:theme legcons:Schedule .

C2024A00060:45 a legcons:Schedule,
        owl:Class,
        dcat:Resource ;
    rdfs:label "Schedule - S45 Schedule 4 Application saving and transitional provisionsoperation of old law"@en-AU ;
    dct:isPartOf C2024A00060:3 ;
    dct:isReferencedBy C2024A00060: ;
    rdfs:comment "Schedule 4 Application saving and transitional provisionsoperation of old law - Abrievated Graph Key: S45"@en-AU ;
    skos:definition "Schedule 4 Application saving and transitional provisionsoperation of old law"@en-AU ;
    skos:narrower C2024A00060:3 ;
    skos:prefLabel "Schedule S45"@en-AU ;
    dcat:accessURL <https://www.legislation.gov.au/C2024A00060/asmade/2024-07-09/text/original/epub/OEBPS/document_1/document_1.html#_Toc171517313> ;
    dcat:landingPage "https://www.legislation.gov.au/C2024A00060/asmade/2024-07-09/text/original/epub/OEBPS/document_1/document_1.html#_Toc171517313"^^xsd:anyURI ;
    dcat:theme legcons:Schedule .

C2024A00060:46 a legcons:Part,
        owl:Class,
        dcat:Resource ;
    rdfs:label "Part - P46 Part 1 Definitions"@en-AU ;
    dct:isPartOf C2024A00060:3 ;
    dct:isReferencedBy C2024A00060: ;
    rdfs:comment "Part 1 Definitions - Abrievated Graph Key: P46"@en-AU ;
    skos:definition "Part 1 Definitions"@en-AU ;
    skos:narrower C2024A00060:3 ;
    skos:prefLabel "Part P46"@en-AU ;
    dcat:accessURL <https://www.legislation.gov.au/C2024A00060/asmade/2024-07-09/text/original/epub/OEBPS/document_1/document_1.html#_Toc171517314> ;
    dcat:landingPage "https://www.legislation.gov.au/C2024A00060/asmade/2024-07-09/text/original/epub/OEBPS/document_1/document_1.html#_Toc171517314"^^xsd:anyURI ;
    dcat:theme legcons:Part .

C2024A00060:47 a legcons:Part,
        owl:Class,
        dcat:Resource ;
    rdfs:label "Part - P47 Part 2 Old levies or charges"@en-AU ;
    dct:isPartOf C2024A00060:3 ;
    dct:isReferencedBy C2024A00060: ;
    rdfs:comment "Part 2 Old levies or charges - Abrievated Graph Key: P47"@en-AU ;
    skos:definition "Part 2 Old levies or charges"@en-AU ;
    skos:narrower C2024A00060:3 ;
    skos:prefLabel "Part P47"@en-AU ;
    dcat:accessURL <https://www.legislation.gov.au/C2024A00060/asmade/2024-07-09/text/original/epub/OEBPS/document_1/document_1.html#_Toc171517315> ;
    dcat:landingPage "https://www.legislation.gov.au/C2024A00060/asmade/2024-07-09/text/original/epub/OEBPS/document_1/document_1.html#_Toc171517315"^^xsd:anyURI ;
    dcat:theme legcons:Part .

C2024A00060:48 a legcons:Part,
        owl:Class,
        dcat:Resource ;
    rdfs:label "Part - P48 Part 3 National Residue Survey Special Account"@en-AU ;
    dct:isPartOf C2024A00060:3 ;
    dct:isReferencedBy C2024A00060: ;
    rdfs:comment "Part 3 National Residue Survey Special Account - Abrievated Graph Key: P48"@en-AU ;
    skos:definition "Part 3 National Residue Survey Special Account"@en-AU ;
    skos:narrower C2024A00060:3 ;
    skos:prefLabel "Part P48"@en-AU ;
    dcat:accessURL <https://www.legislation.gov.au/C2024A00060/asmade/2024-07-09/text/original/epub/OEBPS/document_1/document_1.html#_Toc171517316> ;
    dcat:landingPage "https://www.legislation.gov.au/C2024A00060/asmade/2024-07-09/text/original/epub/OEBPS/document_1/document_1.html#_Toc171517316"^^xsd:anyURI ;
    dcat:theme legcons:Part .

C2024A00060:49 a legcons:Part,
        owl:Class,
        dcat:Resource ;
    rdfs:label "Part - P49 Part 4 Some matters under the old Collection Acts"@en-AU ;
    dct:isPartOf C2024A00060:3 ;
    dct:isReferencedBy C2024A00060: ;
    rdfs:comment "Part 4 Some matters under the old Collection Acts - Abrievated Graph Key: P49"@en-AU ;
    skos:definition "Part 4 Some matters under the old Collection Acts"@en-AU ;
    skos:narrower C2024A00060:3 ;
    skos:prefLabel "Part P49"@en-AU ;
    dcat:accessURL <https://www.legislation.gov.au/C2024A00060/asmade/2024-07-09/text/original/epub/OEBPS/document_1/document_1.html#_Toc171517317> ;
    dcat:landingPage "https://www.legislation.gov.au/C2024A00060/asmade/2024-07-09/text/original/epub/OEBPS/document_1/document_1.html#_Toc171517317"^^xsd:anyURI ;
    dcat:theme legcons:Part .

C2024A00060:5 a legcons:Item,
        owl:Class,
        dcat:Resource ;
    rdfs:label "Item - I5 Australian Animal Health Council Live stock Industries Funding Act 1996"@en-AU ;
    dct:isPartOf C2024A00060:3 ;
    dct:isReferencedBy C2024A00060: ;
    rdfs:comment "Australian Animal Health Council Live stock Industries Funding Act 1996 - Abrievated Graph Key: I5"@en-AU ;
    skos:definition "Australian Animal Health Council Live stock Industries Funding Act 1996"@en-AU ;
    skos:narrower C2024A00060:3 ;
    skos:prefLabel "Item I5"@en-AU ;
    dcat:accessURL <https://www.legislation.gov.au/C2024A00060/asmade/2024-07-09/text/original/epub/OEBPS/document_1/document_1.html#_Toc171517265> ;
    dcat:landingPage "https://www.legislation.gov.au/C2024A00060/asmade/2024-07-09/text/original/epub/OEBPS/document_1/document_1.html#_Toc171517265"^^xsd:anyURI ;
    dcat:theme legcons:Item .

C2024A00060:50 a legcons:Part,
        owl:Class,
        dcat:Resource ;
    rdfs:label "Part - P50 Part 5 Other provisions"@en-AU ;
    dct:isPartOf C2024A00060:3 ;
    dct:isReferencedBy C2024A00060: ;
    rdfs:comment "Part 5 Other provisions - Abrievated Graph Key: P50"@en-AU ;
    skos:definition "Part 5 Other provisions"@en-AU ;
    skos:narrower C2024A00060:3 ;
    skos:prefLabel "Part P50"@en-AU ;
    dcat:accessURL <https://www.legislation.gov.au/C2024A00060/asmade/2024-07-09/text/original/epub/OEBPS/document_1/document_1.html#_Toc171517318> ;
    dcat:landingPage "https://www.legislation.gov.au/C2024A00060/asmade/2024-07-09/text/original/epub/OEBPS/document_1/document_1.html#_Toc171517318"^^xsd:anyURI ;
    dcat:theme legcons:Part .

C2024A00060:6 a legcons:Item,
        owl:Class,
        dcat:Resource ;
    rdfs:label "Item - I6 Australian Meat and Live stock Industry Act 1997"@en-AU ;
    dct:isPartOf C2024A00060:3 ;
    dct:isReferencedBy C2024A00060: ;
    rdfs:comment "Australian Meat and Live stock Industry Act 1997 - Abrievated Graph Key: I6"@en-AU ;
    skos:definition "Australian Meat and Live stock Industry Act 1997"@en-AU ;
    skos:narrower C2024A00060:3 ;
    skos:prefLabel "Item I6"@en-AU ;
    dcat:accessURL <https://www.legislation.gov.au/C2024A00060/asmade/2024-07-09/text/original/epub/OEBPS/document_1/document_1.html#_Toc171517266> ;
    dcat:landingPage "https://www.legislation.gov.au/C2024A00060/asmade/2024-07-09/text/original/epub/OEBPS/document_1/document_1.html#_Toc171517266"^^xsd:anyURI ;
    dcat:theme legcons:Item .

C2024A00060:7 a legcons:Item,
        owl:Class,
        dcat:Resource ;
    rdfs:label "Item - I7 Dairy Adjustment Levy Termination Act 2008"@en-AU ;
    dct:isPartOf C2024A00060:3 ;
    dct:isReferencedBy C2024A00060: ;
    rdfs:comment "Dairy Adjustment Levy Termination Act 2008 - Abrievated Graph Key: I7"@en-AU ;
    skos:definition "Dairy Adjustment Levy Termination Act 2008"@en-AU ;
    skos:narrower C2024A00060:3 ;
    skos:prefLabel "Item I7"@en-AU ;
    dcat:accessURL <https://www.legislation.gov.au/C2024A00060/asmade/2024-07-09/text/original/epub/OEBPS/document_1/document_1.html#_Toc171517267> ;
    dcat:landingPage "https://www.legislation.gov.au/C2024A00060/asmade/2024-07-09/text/original/epub/OEBPS/document_1/document_1.html#_Toc171517267"^^xsd:anyURI ;
    dcat:theme legcons:Item .

C2024A00060:8 a legcons:Item,
        owl:Class,
        dcat:Resource ;
    rdfs:label "Item - I8 Dairy Industry Adjustment Act 2000"@en-AU ;
    dct:isPartOf C2024A00060:3 ;
    dct:isReferencedBy C2024A00060: ;
    rdfs:comment "Dairy Industry Adjustment Act 2000 - Abrievated Graph Key: I8"@en-AU ;
    skos:definition "Dairy Industry Adjustment Act 2000"@en-AU ;
    skos:narrower C2024A00060:3 ;
    skos:prefLabel "Item I8"@en-AU ;
    dcat:accessURL <https://www.legislation.gov.au/C2024A00060/asmade/2024-07-09/text/original/epub/OEBPS/document_1/document_1.html#_Toc171517268> ;
    dcat:landingPage "https://www.legislation.gov.au/C2024A00060/asmade/2024-07-09/text/original/epub/OEBPS/document_1/document_1.html#_Toc171517268"^^xsd:anyURI ;
    dcat:theme legcons:Item .

C2024A00060:9 a legcons:Item,
        owl:Class,
        dcat:Resource ;
    rdfs:label "Item - I9 Dairy Produce Act 1986"@en-AU ;
    dct:isPartOf C2024A00060:3 ;
    dct:isReferencedBy C2024A00060: ;
    rdfs:comment "Dairy Produce Act 1986 - Abrievated Graph Key: I9"@en-AU ;
    skos:definition "Dairy Produce Act 1986"@en-AU ;
    skos:narrower C2024A00060:3 ;
    skos:prefLabel "Item I9"@en-AU ;
    dcat:accessURL <https://www.legislation.gov.au/C2024A00060/asmade/2024-07-09/text/original/epub/OEBPS/document_1/document_1.html#_Toc171517269> ;
    dcat:landingPage "https://www.legislation.gov.au/C2024A00060/asmade/2024-07-09/text/original/epub/OEBPS/document_1/document_1.html#_Toc171517269"^^xsd:anyURI ;
    dcat:theme legcons:Item .

C2024A00060: a owl:Class,
        dcat:Dataset,
        dcat:Resource ;
    rdfs:label "Primary Industries (Consequential Amendments and Transitional Provisions) Act 2024" ;
    dct:Jurisdiction " Department of Agriculture, Fisheries and Forestry "@en-AU ;
    dct:created "2024-08-30T15:21:48.774217"^^xsd:dateTime ;
    dct:creator "https://orcid.org/0009-0007-8434-7325"^^xsd:anyURI ;
    dct:date "2024-07-09T00:00:00+10:00"^^xsd:dateTime ;
    dct:description "Primary Industries (Consequential Amendments and Transitional Provisions) Act 2024"@en-AU ;
    dct:identifier "https://www.legislation.gov.au/C2024A00060/asmade"^^xsd:anyURI ;
    dct:license <https://creativecommons.org/licenses/by-sa/4.0/> ;
    dct:source "scheme=AGLSTERMS.AglsAgent; corporateName=Office Parliamentary Counsel; address=Locked Bag 30 Kingston ACT 2604; contact=+61 2 6120 1400"@en-AU ;
    dct:subject "Primary Industries (Consequential Amendments and Transitional Provisions) Act 2024"@en-AU ;
    dct:title "Primary Industries (Consequential Amendments and Transitional Provisions) Act 2024"@en-AU ;
    owl:imports legcons: ;
    dcat:theme legcons:Item,
        legcons:Part,
        legcons:Schedule ;
    schema:identifier "C2024A00060" ;
    schema:status "In force" ;
    schema:version "C2024A00060" .

C2024A00060:3 a legcons:Item,
        owl:Class,
        dcat:Resource ;
    rdfs:label "Item - I3 3  Schedules"@en-AU ;
    dct:hasPart C2024A00060:10,
        C2024A00060:11,
        C2024A00060:12,
        C2024A00060:13,
        C2024A00060:14,
        C2024A00060:15,
        C2024A00060:16,
        C2024A00060:17,
        C2024A00060:18,
        C2024A00060:19,
        C2024A00060:20,
        C2024A00060:21,
        C2024A00060:22,
        C2024A00060:23,
        C2024A00060:24,
        C2024A00060:25,
        C2024A00060:26,
        C2024A00060:27,
        C2024A00060:28,
        C2024A00060:29,
        C2024A00060:30,
        C2024A00060:31,
        C2024A00060:32,
        C2024A00060:33,
        C2024A00060:34,
        C2024A00060:35,
        C2024A00060:36,
        C2024A00060:37,
        C2024A00060:38,
        C2024A00060:39,
        C2024A00060:4,
        C2024A00060:40,
        C2024A00060:41,
        C2024A00060:42,
        C2024A00060:43,
        C2024A00060:44,
        C2024A00060:45,
        C2024A00060:46,
        C2024A00060:47,
        C2024A00060:48,
        C2024A00060:49,
        C2024A00060:5,
        C2024A00060:50,
        C2024A00060:6,
        C2024A00060:7,
        C2024A00060:8,
        C2024A00060:9 ;
    dct:isReferencedBy C2024A00060: ;
    rdfs:comment "3  Schedules - Abrievated Graph Key: I3"@en-AU ;
    skos:broader C2024A00060:10,
        C2024A00060:11,
        C2024A00060:12,
        C2024A00060:13,
        C2024A00060:14,
        C2024A00060:15,
        C2024A00060:16,
        C2024A00060:17,
        C2024A00060:18,
        C2024A00060:19,
        C2024A00060:20,
        C2024A00060:21,
        C2024A00060:22,
        C2024A00060:23,
        C2024A00060:24,
        C2024A00060:25,
        C2024A00060:26,
        C2024A00060:27,
        C2024A00060:28,
        C2024A00060:29,
        C2024A00060:30,
        C2024A00060:31,
        C2024A00060:32,
        C2024A00060:33,
        C2024A00060:34,
        C2024A00060:35,
        C2024A00060:36,
        C2024A00060:37,
        C2024A00060:38,
        C2024A00060:39,
        C2024A00060:4,
        C2024A00060:40,
        C2024A00060:41,
        C2024A00060:42,
        C2024A00060:43,
        C2024A00060:44,
        C2024A00060:45,
        C2024A00060:46,
        C2024A00060:47,
        C2024A00060:48,
        C2024A00060:49,
        C2024A00060:5,
        C2024A00060:50,
        C2024A00060:6,
        C2024A00060:7,
        C2024A00060:8,
        C2024A00060:9 ;
    skos:definition "3  Schedules"@en-AU ;
    skos:prefLabel "Item I3"@en-AU ;
    dcat:accessURL <https://www.legislation.gov.au/C2024A00060/asmade/2024-07-09/text/original/epub/OEBPS/document_1/document_1.html#_Toc171517263> ;
    dcat:landingPage "https://www.legislation.gov.au/C2024A00060/asmade/2024-07-09/text/original/epub/OEBPS/document_1/document_1.html#_Toc171517263"^^xsd:anyURI ;
    dcat:theme legcons:Item .

