@prefix F1998B00137: <http://example.org/au/leg/dataset/F1998B00137/> .
@prefix dcat: <http://www.w3.org/ns/dcat#> .
@prefix dct: <http://purl.org/dc/terms/> .
@prefix legcons: <http://example.org/au/leg/concepts/> .
@prefix owl: <http://www.w3.org/2002/07/owl#> .
@prefix rdfs: <http://www.w3.org/2000/01/rdf-schema#> .
@prefix schema: <https://schema.org/> .
@prefix skos: <http://www.w3.org/2004/02/skos/core#> .
@prefix xsd: <http://www.w3.org/2001/XMLSchema#> .

F1998B00137:10 a legcons:Item,
        owl:Class,
        dcat:Resource ;
    rdfs:label "Item - I10 8  Liability of exporting agents as intermediaries"@en-AU ;
    dct:isPartOf F1998B00137:6 ;
    dct:isReferencedBy F1998B00137: ;
    rdfs:comment "8  Liability of exporting agents as intermediaries - Abrievated Graph Key: I10"@en-AU ;
    skos:definition "8  Liability of exporting agents as intermediaries"@en-AU ;
    skos:narrower F1998B00137:6 ;
    skos:prefLabel "Item I10"@en-AU ;
    dcat:accessURL <https://www.legislation.gov.au/F1998B00137/2024-07-06/2024-07-06/text/original/epub/OEBPS/document_1/document_1.html#_Toc171769243> ;
    dcat:landingPage "https://www.legislation.gov.au/F1998B00137/2024-07-06/2024-07-06/text/original/epub/OEBPS/document_1/document_1.html#_Toc171769243"^^xsd:anyURI ;
    dcat:theme legcons:Item .

F1998B00137:100 a legcons:Item,
        owl:Class,
        dcat:Resource ;
    rdfs:label "Item - I100 92  What must be in return"@en-AU ;
    dct:isPartOf F1998B00137:91 ;
    dct:isReferencedBy F1998B00137: ;
    rdfs:comment "92  What must be in return - Abrievated Graph Key: I100"@en-AU ;
    skos:definition "92  What must be in return"@en-AU ;
    skos:narrower F1998B00137:91 ;
    skos:prefLabel "Item I100"@en-AU ;
    dcat:accessURL <https://www.legislation.gov.au/F1998B00137/2024-07-06/2024-07-06/text/original/epub/OEBPS/document_1/document_1.html#_Toc171769333> ;
    dcat:landingPage "https://www.legislation.gov.au/F1998B00137/2024-07-06/2024-07-06/text/original/epub/OEBPS/document_1/document_1.html#_Toc171769333"^^xsd:anyURI ;
    dcat:theme legcons:Item .

F1998B00137:101 a legcons:Item,
        owl:Class,
        dcat:Resource ;
    rdfs:label "Item - I101 93  When and how return must be given to Secretary"@en-AU ;
    dct:isPartOf F1998B00137:91 ;
    dct:isReferencedBy F1998B00137: ;
    rdfs:comment "93  When and how return must be given to Secretary - Abrievated Graph Key: I101"@en-AU ;
    skos:definition "93  When and how return must be given to Secretary"@en-AU ;
    skos:narrower F1998B00137:91 ;
    skos:prefLabel "Item I101"@en-AU ;
    dcat:accessURL <https://www.legislation.gov.au/F1998B00137/2024-07-06/2024-07-06/text/original/epub/OEBPS/document_1/document_1.html#_Toc171769334> ;
    dcat:landingPage "https://www.legislation.gov.au/F1998B00137/2024-07-06/2024-07-06/text/original/epub/OEBPS/document_1/document_1.html#_Toc171769334"^^xsd:anyURI ;
    dcat:theme legcons:Item .

F1998B00137:102 a legcons:Item,
        owl:Class,
        dcat:Resource ;
    rdfs:label "Item - I102 94  What records must be kept"@en-AU ;
    dct:isPartOf F1998B00137:91 ;
    dct:isReferencedBy F1998B00137: ;
    rdfs:comment "94  What records must be kept - Abrievated Graph Key: I102"@en-AU ;
    skos:definition "94  What records must be kept"@en-AU ;
    skos:narrower F1998B00137:91 ;
    skos:prefLabel "Item I102"@en-AU ;
    dcat:accessURL <https://www.legislation.gov.au/F1998B00137/2024-07-06/2024-07-06/text/original/epub/OEBPS/document_1/document_1.html#_Toc171769335> ;
    dcat:landingPage "https://www.legislation.gov.au/F1998B00137/2024-07-06/2024-07-06/text/original/epub/OEBPS/document_1/document_1.html#_Toc171769335"^^xsd:anyURI ;
    dcat:theme legcons:Item .

F1998B00137:103 a legcons:Item,
        owl:Class,
        dcat:Resource ;
    rdfs:label "Item - I103 95  How long records must be retained"@en-AU ;
    dct:isPartOf F1998B00137:91 ;
    dct:isReferencedBy F1998B00137: ;
    rdfs:comment "95  How long records must be retained - Abrievated Graph Key: I103"@en-AU ;
    skos:definition "95  How long records must be retained"@en-AU ;
    skos:narrower F1998B00137:91 ;
    skos:prefLabel "Item I103"@en-AU ;
    dcat:accessURL <https://www.legislation.gov.au/F1998B00137/2024-07-06/2024-07-06/text/original/epub/OEBPS/document_1/document_1.html#_Toc171769336> ;
    dcat:landingPage "https://www.legislation.gov.au/F1998B00137/2024-07-06/2024-07-06/text/original/epub/OEBPS/document_1/document_1.html#_Toc171769336"^^xsd:anyURI ;
    dcat:theme legcons:Item .

F1998B00137:104 a legcons:Item,
        owl:Class,
        dcat:Resource ;
    rdfs:label "Item - I104 96  Transitionalobligations about returns under former Regulations"@en-AU ;
    dct:isPartOf F1998B00137:91 ;
    dct:isReferencedBy F1998B00137: ;
    rdfs:comment "96  Transitionalobligations about returns under former Regulations - Abrievated Graph Key: I104"@en-AU ;
    skos:definition "96  Transitionalobligations about returns under former Regulations"@en-AU ;
    skos:narrower F1998B00137:91 ;
    skos:prefLabel "Item I104"@en-AU ;
    dcat:accessURL <https://www.legislation.gov.au/F1998B00137/2024-07-06/2024-07-06/text/original/epub/OEBPS/document_1/document_1.html#_Toc171769337> ;
    dcat:landingPage "https://www.legislation.gov.au/F1998B00137/2024-07-06/2024-07-06/text/original/epub/OEBPS/document_1/document_1.html#_Toc171769337"^^xsd:anyURI ;
    dcat:theme legcons:Item .

F1998B00137:107 a legcons:Item,
        owl:Class,
        dcat:Resource ;
    rdfs:label "Item - I107 97  Meaning of expressions for Part"@en-AU ;
    dct:isPartOf F1998B00137:106 ;
    dct:isReferencedBy F1998B00137: ;
    rdfs:comment "97  Meaning of expressions for Part - Abrievated Graph Key: I107"@en-AU ;
    skos:definition "97  Meaning of expressions for Part"@en-AU ;
    skos:narrower F1998B00137:106 ;
    skos:prefLabel "Item I107"@en-AU ;
    dcat:accessURL <https://www.legislation.gov.au/F1998B00137/2024-07-06/2024-07-06/text/original/epub/OEBPS/document_1/document_1.html#_Toc171769340> ;
    dcat:landingPage "https://www.legislation.gov.au/F1998B00137/2024-07-06/2024-07-06/text/original/epub/OEBPS/document_1/document_1.html#_Toc171769340"^^xsd:anyURI ;
    dcat:theme legcons:Item .

F1998B00137:108 a legcons:Division,
        owl:Class,
        dcat:Resource ;
    rdfs:label "Division - D108 Division 2 Potatoes"@en-AU ;
    dct:isPartOf F1998B00137:105 ;
    dct:isReferencedBy F1998B00137: ;
    rdfs:comment "Division 2 Potatoes - Abrievated Graph Key: D108"@en-AU ;
    skos:definition "Division 2 Potatoes"@en-AU ;
    skos:narrower F1998B00137:105 ;
    skos:prefLabel "Division D108"@en-AU ;
    dcat:accessURL <https://www.legislation.gov.au/F1998B00137/2024-07-06/2024-07-06/text/original/epub/OEBPS/document_1/document_1.html#_Toc171769341> ;
    dcat:landingPage "https://www.legislation.gov.au/F1998B00137/2024-07-06/2024-07-06/text/original/epub/OEBPS/document_1/document_1.html#_Toc171769341"^^xsd:anyURI ;
    dcat:theme legcons:Division .

F1998B00137:109 a legcons:Item,
        owl:Class,
        dcat:Resource ;
    rdfs:label "Item - I109 98  Meaning of expressions for Division"@en-AU ;
    dct:isPartOf F1998B00137:105 ;
    dct:isReferencedBy F1998B00137: ;
    rdfs:comment "98  Meaning of expressions for Division - Abrievated Graph Key: I109"@en-AU ;
    skos:definition "98  Meaning of expressions for Division"@en-AU ;
    skos:narrower F1998B00137:105 ;
    skos:prefLabel "Item I109"@en-AU ;
    dcat:accessURL <https://www.legislation.gov.au/F1998B00137/2024-07-06/2024-07-06/text/original/epub/OEBPS/document_1/document_1.html#_Toc171769342> ;
    dcat:landingPage "https://www.legislation.gov.au/F1998B00137/2024-07-06/2024-07-06/text/original/epub/OEBPS/document_1/document_1.html#_Toc171769342"^^xsd:anyURI ;
    dcat:theme legcons:Item .

F1998B00137:11 a legcons:Item,
        owl:Class,
        dcat:Resource ;
    rdfs:label "Item - I11 9  Rate of NRS customs levy on export of aquatic animals"@en-AU ;
    dct:isPartOf F1998B00137:6 ;
    dct:isReferencedBy F1998B00137: ;
    rdfs:comment "9  Rate of NRS customs levy on export of aquatic animals - Abrievated Graph Key: I11"@en-AU ;
    skos:definition "9  Rate of NRS customs levy on export of aquatic animals"@en-AU ;
    skos:narrower F1998B00137:6 ;
    skos:prefLabel "Item I11"@en-AU ;
    dcat:accessURL <https://www.legislation.gov.au/F1998B00137/2024-07-06/2024-07-06/text/original/epub/OEBPS/document_1/document_1.html#_Toc171769244> ;
    dcat:landingPage "https://www.legislation.gov.au/F1998B00137/2024-07-06/2024-07-06/text/original/epub/OEBPS/document_1/document_1.html#_Toc171769244"^^xsd:anyURI ;
    dcat:theme legcons:Item .

F1998B00137:110 a legcons:Item,
        owl:Class,
        dcat:Resource ;
    rdfs:label "Item - I110 99  Incorporation with Part 14 of Schedule 22 to the Collection Regulations"@en-AU ;
    dct:isPartOf F1998B00137:105 ;
    dct:isReferencedBy F1998B00137: ;
    rdfs:comment "99  Incorporation with Part 14 of Schedule 22 to the Collection Regulations - Abrievated Graph Key: I110"@en-AU ;
    skos:definition "99  Incorporation with Part 14 of Schedule 22 to the Collection Regulations"@en-AU ;
    skos:narrower F1998B00137:105 ;
    skos:prefLabel "Item I110"@en-AU ;
    dcat:accessURL <https://www.legislation.gov.au/F1998B00137/2024-07-06/2024-07-06/text/original/epub/OEBPS/document_1/document_1.html#_Toc171769343> ;
    dcat:landingPage "https://www.legislation.gov.au/F1998B00137/2024-07-06/2024-07-06/text/original/epub/OEBPS/document_1/document_1.html#_Toc171769343"^^xsd:anyURI ;
    dcat:theme legcons:Item .

F1998B00137:111 a legcons:Item,
        owl:Class,
        dcat:Resource ;
    rdfs:label "Item - I111 101  When levy is due for payment Collection Act s 6"@en-AU ;
    dct:isPartOf F1998B00137:105 ;
    dct:isReferencedBy F1998B00137: ;
    rdfs:comment "101  When levy is due for payment Collection Act s 6 - Abrievated Graph Key: I111"@en-AU ;
    skos:definition "101  When levy is due for payment Collection Act s 6"@en-AU ;
    skos:narrower F1998B00137:105 ;
    skos:prefLabel "Item I111"@en-AU ;
    dcat:accessURL <https://www.legislation.gov.au/F1998B00137/2024-07-06/2024-07-06/text/original/epub/OEBPS/document_1/document_1.html#_Toc171769344> ;
    dcat:landingPage "https://www.legislation.gov.au/F1998B00137/2024-07-06/2024-07-06/text/original/epub/OEBPS/document_1/document_1.html#_Toc171769344"^^xsd:anyURI ;
    dcat:theme legcons:Item .

F1998B00137:112 a legcons:Item,
        owl:Class,
        dcat:Resource ;
    rdfs:label "Item - I112 102  Information in returns under Part 14 of Schedule 22 to the Collection Regulations"@en-AU ;
    dct:isPartOf F1998B00137:105 ;
    dct:isReferencedBy F1998B00137: ;
    rdfs:comment "102  Information in returns under Part 14 of Schedule 22 to the Collection Regulations - Abrievated Graph Key: I112"@en-AU ;
    skos:definition "102  Information in returns under Part 14 of Schedule 22 to the Collection Regulations"@en-AU ;
    skos:narrower F1998B00137:105 ;
    skos:prefLabel "Item I112"@en-AU ;
    dcat:accessURL <https://www.legislation.gov.au/F1998B00137/2024-07-06/2024-07-06/text/original/epub/OEBPS/document_1/document_1.html#_Toc171769345> ;
    dcat:landingPage "https://www.legislation.gov.au/F1998B00137/2024-07-06/2024-07-06/text/original/epub/OEBPS/document_1/document_1.html#_Toc171769345"^^xsd:anyURI ;
    dcat:theme legcons:Item .

F1998B00137:113 a legcons:Item,
        owl:Class,
        dcat:Resource ;
    rdfs:label "Item - I113 103  Information in records under Part 14 of Schedule 22 to the Collection Regulations"@en-AU ;
    dct:isPartOf F1998B00137:105 ;
    dct:isReferencedBy F1998B00137: ;
    rdfs:comment "103  Information in records under Part 14 of Schedule 22 to the Collection Regulations - Abrievated Graph Key: I113"@en-AU ;
    skos:definition "103  Information in records under Part 14 of Schedule 22 to the Collection Regulations"@en-AU ;
    skos:narrower F1998B00137:105 ;
    skos:prefLabel "Item I113"@en-AU ;
    dcat:accessURL <https://www.legislation.gov.au/F1998B00137/2024-07-06/2024-07-06/text/original/epub/OEBPS/document_1/document_1.html#_Toc171769346> ;
    dcat:landingPage "https://www.legislation.gov.au/F1998B00137/2024-07-06/2024-07-06/text/original/epub/OEBPS/document_1/document_1.html#_Toc171769346"^^xsd:anyURI ;
    dcat:theme legcons:Item .

F1998B00137:114 a legcons:Division,
        owl:Class,
        dcat:Resource ;
    rdfs:label "Division - D114 Division 3 Onions"@en-AU ;
    dct:isPartOf F1998B00137:105 ;
    dct:isReferencedBy F1998B00137: ;
    rdfs:comment "Division 3 Onions - Abrievated Graph Key: D114"@en-AU ;
    skos:definition "Division 3 Onions"@en-AU ;
    skos:narrower F1998B00137:105 ;
    skos:prefLabel "Division D114"@en-AU ;
    dcat:accessURL <https://www.legislation.gov.au/F1998B00137/2024-07-06/2024-07-06/text/original/epub/OEBPS/document_1/document_1.html#_Toc171769347> ;
    dcat:landingPage "https://www.legislation.gov.au/F1998B00137/2024-07-06/2024-07-06/text/original/epub/OEBPS/document_1/document_1.html#_Toc171769347"^^xsd:anyURI ;
    dcat:theme legcons:Division .

F1998B00137:115 a legcons:Item,
        owl:Class,
        dcat:Resource ;
    rdfs:label "Item - I115 104  Meaning of expressions for Division"@en-AU ;
    dct:isPartOf F1998B00137:105 ;
    dct:isReferencedBy F1998B00137: ;
    rdfs:comment "104  Meaning of expressions for Division - Abrievated Graph Key: I115"@en-AU ;
    skos:definition "104  Meaning of expressions for Division"@en-AU ;
    skos:narrower F1998B00137:105 ;
    skos:prefLabel "Item I115"@en-AU ;
    dcat:accessURL <https://www.legislation.gov.au/F1998B00137/2024-07-06/2024-07-06/text/original/epub/OEBPS/document_1/document_1.html#_Toc171769348> ;
    dcat:landingPage "https://www.legislation.gov.au/F1998B00137/2024-07-06/2024-07-06/text/original/epub/OEBPS/document_1/document_1.html#_Toc171769348"^^xsd:anyURI ;
    dcat:theme legcons:Item .

F1998B00137:116 a legcons:Item,
        owl:Class,
        dcat:Resource ;
    rdfs:label "Item - I116 105  Levy year Collection Act s 41 definition of levy year"@en-AU ;
    dct:isPartOf F1998B00137:105 ;
    dct:isReferencedBy F1998B00137: ;
    rdfs:comment "105  Levy year Collection Act s 41 definition of levy year - Abrievated Graph Key: I116"@en-AU ;
    skos:definition "105  Levy year Collection Act s 41 definition of levy year"@en-AU ;
    skos:narrower F1998B00137:105 ;
    skos:prefLabel "Item I116"@en-AU ;
    dcat:accessURL <https://www.legislation.gov.au/F1998B00137/2024-07-06/2024-07-06/text/original/epub/OEBPS/document_1/document_1.html#_Toc171769349> ;
    dcat:landingPage "https://www.legislation.gov.au/F1998B00137/2024-07-06/2024-07-06/text/original/epub/OEBPS/document_1/document_1.html#_Toc171769349"^^xsd:anyURI ;
    dcat:theme legcons:Item .

F1998B00137:117 a legcons:Item,
        owl:Class,
        dcat:Resource ;
    rdfs:label "Item - I117 106  Owner etc and exporter are producers for Collection Act"@en-AU ;
    dct:isPartOf F1998B00137:105 ;
    dct:isReferencedBy F1998B00137: ;
    rdfs:comment "106  Owner etc and exporter are producers for Collection Act - Abrievated Graph Key: I117"@en-AU ;
    skos:definition "106  Owner etc and exporter are producers for Collection Act"@en-AU ;
    skos:narrower F1998B00137:105 ;
    skos:prefLabel "Item I117"@en-AU ;
    dcat:accessURL <https://www.legislation.gov.au/F1998B00137/2024-07-06/2024-07-06/text/original/epub/OEBPS/document_1/document_1.html#_Toc171769350> ;
    dcat:landingPage "https://www.legislation.gov.au/F1998B00137/2024-07-06/2024-07-06/text/original/epub/OEBPS/document_1/document_1.html#_Toc171769350"^^xsd:anyURI ;
    dcat:theme legcons:Item .

F1998B00137:118 a legcons:Item,
        owl:Class,
        dcat:Resource ;
    rdfs:label "Item - I118 107  Liability of processor as intermediary"@en-AU ;
    dct:isPartOf F1998B00137:105 ;
    dct:isReferencedBy F1998B00137: ;
    rdfs:comment "107  Liability of processor as intermediary - Abrievated Graph Key: I118"@en-AU ;
    skos:definition "107  Liability of processor as intermediary"@en-AU ;
    skos:narrower F1998B00137:105 ;
    skos:prefLabel "Item I118"@en-AU ;
    dcat:accessURL <https://www.legislation.gov.au/F1998B00137/2024-07-06/2024-07-06/text/original/epub/OEBPS/document_1/document_1.html#_Toc171769351> ;
    dcat:landingPage "https://www.legislation.gov.au/F1998B00137/2024-07-06/2024-07-06/text/original/epub/OEBPS/document_1/document_1.html#_Toc171769351"^^xsd:anyURI ;
    dcat:theme legcons:Item .

F1998B00137:119 a legcons:Item,
        owl:Class,
        dcat:Resource ;
    rdfs:label "Item - I119 108  Rate of NRS customs levy on onions"@en-AU ;
    dct:isPartOf F1998B00137:105 ;
    dct:isReferencedBy F1998B00137: ;
    rdfs:comment "108  Rate of NRS customs levy on onions - Abrievated Graph Key: I119"@en-AU ;
    skos:definition "108  Rate of NRS customs levy on onions"@en-AU ;
    skos:narrower F1998B00137:105 ;
    skos:prefLabel "Item I119"@en-AU ;
    dcat:accessURL <https://www.legislation.gov.au/F1998B00137/2024-07-06/2024-07-06/text/original/epub/OEBPS/document_1/document_1.html#_Toc171769352> ;
    dcat:landingPage "https://www.legislation.gov.au/F1998B00137/2024-07-06/2024-07-06/text/original/epub/OEBPS/document_1/document_1.html#_Toc171769352"^^xsd:anyURI ;
    dcat:theme legcons:Item .

F1998B00137:12 a legcons:Item,
        owl:Class,
        dcat:Resource ;
    rdfs:label "Item - I12 10  When levy is due for payment Collection Act s 6"@en-AU ;
    dct:isPartOf F1998B00137:6 ;
    dct:isReferencedBy F1998B00137: ;
    rdfs:comment "10  When levy is due for payment Collection Act s 6 - Abrievated Graph Key: I12"@en-AU ;
    skos:definition "10  When levy is due for payment Collection Act s 6"@en-AU ;
    skos:narrower F1998B00137:6 ;
    skos:prefLabel "Item I12"@en-AU ;
    dcat:accessURL <https://www.legislation.gov.au/F1998B00137/2024-07-06/2024-07-06/text/original/epub/OEBPS/document_1/document_1.html#_Toc171769245> ;
    dcat:landingPage "https://www.legislation.gov.au/F1998B00137/2024-07-06/2024-07-06/text/original/epub/OEBPS/document_1/document_1.html#_Toc171769245"^^xsd:anyURI ;
    dcat:theme legcons:Item .

F1998B00137:120 a legcons:Item,
        owl:Class,
        dcat:Resource ;
    rdfs:label "Item - I120 109  Rate of NRS excise levy on onions"@en-AU ;
    dct:isPartOf F1998B00137:105 ;
    dct:isReferencedBy F1998B00137: ;
    rdfs:comment "109  Rate of NRS excise levy on onions - Abrievated Graph Key: I120"@en-AU ;
    skos:definition "109  Rate of NRS excise levy on onions"@en-AU ;
    skos:narrower F1998B00137:105 ;
    skos:prefLabel "Item I120"@en-AU ;
    dcat:accessURL <https://www.legislation.gov.au/F1998B00137/2024-07-06/2024-07-06/text/original/epub/OEBPS/document_1/document_1.html#_Toc171769353> ;
    dcat:landingPage "https://www.legislation.gov.au/F1998B00137/2024-07-06/2024-07-06/text/original/epub/OEBPS/document_1/document_1.html#_Toc171769353"^^xsd:anyURI ;
    dcat:theme legcons:Item .

F1998B00137:121 a legcons:Item,
        owl:Class,
        dcat:Resource ;
    rdfs:label "Item - I121 110  When levy is due for payment Collection Act s 6"@en-AU ;
    dct:isPartOf F1998B00137:105 ;
    dct:isReferencedBy F1998B00137: ;
    rdfs:comment "110  When levy is due for payment Collection Act s 6 - Abrievated Graph Key: I121"@en-AU ;
    skos:definition "110  When levy is due for payment Collection Act s 6"@en-AU ;
    skos:narrower F1998B00137:105 ;
    skos:prefLabel "Item I121"@en-AU ;
    dcat:accessURL <https://www.legislation.gov.au/F1998B00137/2024-07-06/2024-07-06/text/original/epub/OEBPS/document_1/document_1.html#_Toc171769354> ;
    dcat:landingPage "https://www.legislation.gov.au/F1998B00137/2024-07-06/2024-07-06/text/original/epub/OEBPS/document_1/document_1.html#_Toc171769354"^^xsd:anyURI ;
    dcat:theme legcons:Item .

F1998B00137:122 a legcons:Item,
        owl:Class,
        dcat:Resource ;
    rdfs:label "Item - I122 111  Who must give Secretary quarterly return"@en-AU ;
    dct:isPartOf F1998B00137:105 ;
    dct:isReferencedBy F1998B00137: ;
    rdfs:comment "111  Who must give Secretary quarterly return - Abrievated Graph Key: I122"@en-AU ;
    skos:definition "111  Who must give Secretary quarterly return"@en-AU ;
    skos:narrower F1998B00137:105 ;
    skos:prefLabel "Item I122"@en-AU ;
    dcat:accessURL <https://www.legislation.gov.au/F1998B00137/2024-07-06/2024-07-06/text/original/epub/OEBPS/document_1/document_1.html#_Toc171769355> ;
    dcat:landingPage "https://www.legislation.gov.au/F1998B00137/2024-07-06/2024-07-06/text/original/epub/OEBPS/document_1/document_1.html#_Toc171769355"^^xsd:anyURI ;
    dcat:theme legcons:Item .

F1998B00137:123 a legcons:Item,
        owl:Class,
        dcat:Resource ;
    rdfs:label "Item - I123 112  Applications for exemptions from giving Secretary quarterly returns"@en-AU ;
    dct:isPartOf F1998B00137:105 ;
    dct:isReferencedBy F1998B00137: ;
    rdfs:comment "112  Applications for exemptions from giving Secretary quarterly returns - Abrievated Graph Key: I123"@en-AU ;
    skos:definition "112  Applications for exemptions from giving Secretary quarterly returns"@en-AU ;
    skos:narrower F1998B00137:105 ;
    skos:prefLabel "Item I123"@en-AU ;
    dcat:accessURL <https://www.legislation.gov.au/F1998B00137/2024-07-06/2024-07-06/text/original/epub/OEBPS/document_1/document_1.html#_Toc171769356> ;
    dcat:landingPage "https://www.legislation.gov.au/F1998B00137/2024-07-06/2024-07-06/text/original/epub/OEBPS/document_1/document_1.html#_Toc171769356"^^xsd:anyURI ;
    dcat:theme legcons:Item .

F1998B00137:124 a legcons:Item,
        owl:Class,
        dcat:Resource ;
    rdfs:label "Item - I124 113  How to apply for exemption"@en-AU ;
    dct:isPartOf F1998B00137:105 ;
    dct:isReferencedBy F1998B00137: ;
    rdfs:comment "113  How to apply for exemption - Abrievated Graph Key: I124"@en-AU ;
    skos:definition "113  How to apply for exemption"@en-AU ;
    skos:narrower F1998B00137:105 ;
    skos:prefLabel "Item I124"@en-AU ;
    dcat:accessURL <https://www.legislation.gov.au/F1998B00137/2024-07-06/2024-07-06/text/original/epub/OEBPS/document_1/document_1.html#_Toc171769357> ;
    dcat:landingPage "https://www.legislation.gov.au/F1998B00137/2024-07-06/2024-07-06/text/original/epub/OEBPS/document_1/document_1.html#_Toc171769357"^^xsd:anyURI ;
    dcat:theme legcons:Item .

F1998B00137:125 a legcons:Item,
        owl:Class,
        dcat:Resource ;
    rdfs:label "Item - I125 114  Grant or refusal of exemption"@en-AU ;
    dct:isPartOf F1998B00137:105 ;
    dct:isReferencedBy F1998B00137: ;
    rdfs:comment "114  Grant or refusal of exemption - Abrievated Graph Key: I125"@en-AU ;
    skos:definition "114  Grant or refusal of exemption"@en-AU ;
    skos:narrower F1998B00137:105 ;
    skos:prefLabel "Item I125"@en-AU ;
    dcat:accessURL <https://www.legislation.gov.au/F1998B00137/2024-07-06/2024-07-06/text/original/epub/OEBPS/document_1/document_1.html#_Toc171769358> ;
    dcat:landingPage "https://www.legislation.gov.au/F1998B00137/2024-07-06/2024-07-06/text/original/epub/OEBPS/document_1/document_1.html#_Toc171769358"^^xsd:anyURI ;
    dcat:theme legcons:Item .

F1998B00137:126 a legcons:Item,
        owl:Class,
        dcat:Resource ;
    rdfs:label "Item - I126 115  Continuation of exemption"@en-AU ;
    dct:isPartOf F1998B00137:105 ;
    dct:isReferencedBy F1998B00137: ;
    rdfs:comment "115  Continuation of exemption - Abrievated Graph Key: I126"@en-AU ;
    skos:definition "115  Continuation of exemption"@en-AU ;
    skos:narrower F1998B00137:105 ;
    skos:prefLabel "Item I126"@en-AU ;
    dcat:accessURL <https://www.legislation.gov.au/F1998B00137/2024-07-06/2024-07-06/text/original/epub/OEBPS/document_1/document_1.html#_Toc171769359> ;
    dcat:landingPage "https://www.legislation.gov.au/F1998B00137/2024-07-06/2024-07-06/text/original/epub/OEBPS/document_1/document_1.html#_Toc171769359"^^xsd:anyURI ;
    dcat:theme legcons:Item .

F1998B00137:127 a legcons:Item,
        owl:Class,
        dcat:Resource ;
    rdfs:label "Item - I127 116  What Secretary must consider when deciding whether to grant or continue exemption"@en-AU ;
    dct:isPartOf F1998B00137:105 ;
    dct:isReferencedBy F1998B00137: ;
    rdfs:comment "116  What Secretary must consider when deciding whether to grant or continue exemption - Abrievated Graph Key: I127"@en-AU ;
    skos:definition "116  What Secretary must consider when deciding whether to grant or continue exemption"@en-AU ;
    skos:narrower F1998B00137:105 ;
    skos:prefLabel "Item I127"@en-AU ;
    dcat:accessURL <https://www.legislation.gov.au/F1998B00137/2024-07-06/2024-07-06/text/original/epub/OEBPS/document_1/document_1.html#_Toc171769360> ;
    dcat:landingPage "https://www.legislation.gov.au/F1998B00137/2024-07-06/2024-07-06/text/original/epub/OEBPS/document_1/document_1.html#_Toc171769360"^^xsd:anyURI ;
    dcat:theme legcons:Item .

F1998B00137:128 a legcons:Item,
        owl:Class,
        dcat:Resource ;
    rdfs:label "Item - I128 117  Who must give Secretary annual return"@en-AU ;
    dct:isPartOf F1998B00137:105 ;
    dct:isReferencedBy F1998B00137: ;
    rdfs:comment "117  Who must give Secretary annual return - Abrievated Graph Key: I128"@en-AU ;
    skos:definition "117  Who must give Secretary annual return"@en-AU ;
    skos:narrower F1998B00137:105 ;
    skos:prefLabel "Item I128"@en-AU ;
    dcat:accessURL <https://www.legislation.gov.au/F1998B00137/2024-07-06/2024-07-06/text/original/epub/OEBPS/document_1/document_1.html#_Toc171769361> ;
    dcat:landingPage "https://www.legislation.gov.au/F1998B00137/2024-07-06/2024-07-06/text/original/epub/OEBPS/document_1/document_1.html#_Toc171769361"^^xsd:anyURI ;
    dcat:theme legcons:Item .

F1998B00137:129 a legcons:Item,
        owl:Class,
        dcat:Resource ;
    rdfs:label "Item - I129 118  What must be in return"@en-AU ;
    dct:isPartOf F1998B00137:105 ;
    dct:isReferencedBy F1998B00137: ;
    rdfs:comment "118  What must be in return - Abrievated Graph Key: I129"@en-AU ;
    skos:definition "118  What must be in return"@en-AU ;
    skos:narrower F1998B00137:105 ;
    skos:prefLabel "Item I129"@en-AU ;
    dcat:accessURL <https://www.legislation.gov.au/F1998B00137/2024-07-06/2024-07-06/text/original/epub/OEBPS/document_1/document_1.html#_Toc171769362> ;
    dcat:landingPage "https://www.legislation.gov.au/F1998B00137/2024-07-06/2024-07-06/text/original/epub/OEBPS/document_1/document_1.html#_Toc171769362"^^xsd:anyURI ;
    dcat:theme legcons:Item .

F1998B00137:13 a legcons:Item,
        owl:Class,
        dcat:Resource ;
    rdfs:label "Item - I13 11  Who must give Secretary quarterly returns"@en-AU ;
    dct:isPartOf F1998B00137:6 ;
    dct:isReferencedBy F1998B00137: ;
    rdfs:comment "11  Who must give Secretary quarterly returns - Abrievated Graph Key: I13"@en-AU ;
    skos:definition "11  Who must give Secretary quarterly returns"@en-AU ;
    skos:narrower F1998B00137:6 ;
    skos:prefLabel "Item I13"@en-AU ;
    dcat:accessURL <https://www.legislation.gov.au/F1998B00137/2024-07-06/2024-07-06/text/original/epub/OEBPS/document_1/document_1.html#_Toc171769246> ;
    dcat:landingPage "https://www.legislation.gov.au/F1998B00137/2024-07-06/2024-07-06/text/original/epub/OEBPS/document_1/document_1.html#_Toc171769246"^^xsd:anyURI ;
    dcat:theme legcons:Item .

F1998B00137:130 a legcons:Item,
        owl:Class,
        dcat:Resource ;
    rdfs:label "Item - I130 119  When and how quarterly return must be given to Secretary"@en-AU ;
    dct:isPartOf F1998B00137:105 ;
    dct:isReferencedBy F1998B00137: ;
    rdfs:comment "119  When and how quarterly return must be given to Secretary - Abrievated Graph Key: I130"@en-AU ;
    skos:definition "119  When and how quarterly return must be given to Secretary"@en-AU ;
    skos:narrower F1998B00137:105 ;
    skos:prefLabel "Item I130"@en-AU ;
    dcat:accessURL <https://www.legislation.gov.au/F1998B00137/2024-07-06/2024-07-06/text/original/epub/OEBPS/document_1/document_1.html#_Toc171769363> ;
    dcat:landingPage "https://www.legislation.gov.au/F1998B00137/2024-07-06/2024-07-06/text/original/epub/OEBPS/document_1/document_1.html#_Toc171769363"^^xsd:anyURI ;
    dcat:theme legcons:Item .

F1998B00137:131 a legcons:Item,
        owl:Class,
        dcat:Resource ;
    rdfs:label "Item - I131 120  When and how annual return must be given to Secretary"@en-AU ;
    dct:isPartOf F1998B00137:105 ;
    dct:isReferencedBy F1998B00137: ;
    rdfs:comment "120  When and how annual return must be given to Secretary - Abrievated Graph Key: I131"@en-AU ;
    skos:definition "120  When and how annual return must be given to Secretary"@en-AU ;
    skos:narrower F1998B00137:105 ;
    skos:prefLabel "Item I131"@en-AU ;
    dcat:accessURL <https://www.legislation.gov.au/F1998B00137/2024-07-06/2024-07-06/text/original/epub/OEBPS/document_1/document_1.html#_Toc171769364> ;
    dcat:landingPage "https://www.legislation.gov.au/F1998B00137/2024-07-06/2024-07-06/text/original/epub/OEBPS/document_1/document_1.html#_Toc171769364"^^xsd:anyURI ;
    dcat:theme legcons:Item .

F1998B00137:132 a legcons:Item,
        owl:Class,
        dcat:Resource ;
    rdfs:label "Item - I132 121  What records must be kept"@en-AU ;
    dct:isPartOf F1998B00137:105 ;
    dct:isReferencedBy F1998B00137: ;
    rdfs:comment "121  What records must be kept - Abrievated Graph Key: I132"@en-AU ;
    skos:definition "121  What records must be kept"@en-AU ;
    skos:narrower F1998B00137:105 ;
    skos:prefLabel "Item I132"@en-AU ;
    dcat:accessURL <https://www.legislation.gov.au/F1998B00137/2024-07-06/2024-07-06/text/original/epub/OEBPS/document_1/document_1.html#_Toc171769365> ;
    dcat:landingPage "https://www.legislation.gov.au/F1998B00137/2024-07-06/2024-07-06/text/original/epub/OEBPS/document_1/document_1.html#_Toc171769365"^^xsd:anyURI ;
    dcat:theme legcons:Item .

F1998B00137:133 a legcons:Item,
        owl:Class,
        dcat:Resource ;
    rdfs:label "Item - I133 122  How long records must be retained"@en-AU ;
    dct:isPartOf F1998B00137:105 ;
    dct:isReferencedBy F1998B00137: ;
    rdfs:comment "122  How long records must be retained - Abrievated Graph Key: I133"@en-AU ;
    skos:definition "122  How long records must be retained"@en-AU ;
    skos:narrower F1998B00137:105 ;
    skos:prefLabel "Item I133"@en-AU ;
    dcat:accessURL <https://www.legislation.gov.au/F1998B00137/2024-07-06/2024-07-06/text/original/epub/OEBPS/document_1/document_1.html#_Toc171769366> ;
    dcat:landingPage "https://www.legislation.gov.au/F1998B00137/2024-07-06/2024-07-06/text/original/epub/OEBPS/document_1/document_1.html#_Toc171769366"^^xsd:anyURI ;
    dcat:theme legcons:Item .

F1998B00137:134 a legcons:Item,
        owl:Class,
        dcat:Resource ;
    rdfs:label "Item - I134 123  Review of decisions"@en-AU ;
    dct:isPartOf F1998B00137:105 ;
    dct:isReferencedBy F1998B00137: ;
    rdfs:comment "123  Review of decisions - Abrievated Graph Key: I134"@en-AU ;
    skos:definition "123  Review of decisions"@en-AU ;
    skos:narrower F1998B00137:105 ;
    skos:prefLabel "Item I134"@en-AU ;
    dcat:accessURL <https://www.legislation.gov.au/F1998B00137/2024-07-06/2024-07-06/text/original/epub/OEBPS/document_1/document_1.html#_Toc171769367> ;
    dcat:landingPage "https://www.legislation.gov.au/F1998B00137/2024-07-06/2024-07-06/text/original/epub/OEBPS/document_1/document_1.html#_Toc171769367"^^xsd:anyURI ;
    dcat:theme legcons:Item .

F1998B00137:135 a legcons:Item,
        owl:Class,
        dcat:Resource ;
    rdfs:label "Item - I135 124  Transitionalobligations about returns under former regulations"@en-AU ;
    dct:isPartOf F1998B00137:105 ;
    dct:isReferencedBy F1998B00137: ;
    rdfs:comment "124  Transitionalobligations about returns under former regulations - Abrievated Graph Key: I135"@en-AU ;
    skos:definition "124  Transitionalobligations about returns under former regulations"@en-AU ;
    skos:narrower F1998B00137:105 ;
    skos:prefLabel "Item I135"@en-AU ;
    dcat:accessURL <https://www.legislation.gov.au/F1998B00137/2024-07-06/2024-07-06/text/original/epub/OEBPS/document_1/document_1.html#_Toc171769368> ;
    dcat:landingPage "https://www.legislation.gov.au/F1998B00137/2024-07-06/2024-07-06/text/original/epub/OEBPS/document_1/document_1.html#_Toc171769368"^^xsd:anyURI ;
    dcat:theme legcons:Item .

F1998B00137:136 a legcons:Division,
        owl:Class,
        dcat:Resource ;
    rdfs:label "Division - D136 Division 4 Apples and pears"@en-AU ;
    dct:isPartOf F1998B00137:105 ;
    dct:isReferencedBy F1998B00137: ;
    rdfs:comment "Division 4 Apples and pears - Abrievated Graph Key: D136"@en-AU ;
    skos:definition "Division 4 Apples and pears"@en-AU ;
    skos:narrower F1998B00137:105 ;
    skos:prefLabel "Division D136"@en-AU ;
    dcat:accessURL <https://www.legislation.gov.au/F1998B00137/2024-07-06/2024-07-06/text/original/epub/OEBPS/document_1/document_1.html#_Toc171769369> ;
    dcat:landingPage "https://www.legislation.gov.au/F1998B00137/2024-07-06/2024-07-06/text/original/epub/OEBPS/document_1/document_1.html#_Toc171769369"^^xsd:anyURI ;
    dcat:theme legcons:Division .

F1998B00137:137 a legcons:Item,
        owl:Class,
        dcat:Resource ;
    rdfs:label "Item - I137 125  Meaning of expressions for Division"@en-AU ;
    dct:isPartOf F1998B00137:105 ;
    dct:isReferencedBy F1998B00137: ;
    rdfs:comment "125  Meaning of expressions for Division - Abrievated Graph Key: I137"@en-AU ;
    skos:definition "125  Meaning of expressions for Division"@en-AU ;
    skos:narrower F1998B00137:105 ;
    skos:prefLabel "Item I137"@en-AU ;
    dcat:accessURL <https://www.legislation.gov.au/F1998B00137/2024-07-06/2024-07-06/text/original/epub/OEBPS/document_1/document_1.html#_Toc171769370> ;
    dcat:landingPage "https://www.legislation.gov.au/F1998B00137/2024-07-06/2024-07-06/text/original/epub/OEBPS/document_1/document_1.html#_Toc171769370"^^xsd:anyURI ;
    dcat:theme legcons:Item .

F1998B00137:138 a legcons:Item,
        owl:Class,
        dcat:Resource ;
    rdfs:label "Item - I138 126  Incorporation with Part 3 of Schedule 22 to the Collection Regulations"@en-AU ;
    dct:isPartOf F1998B00137:105 ;
    dct:isReferencedBy F1998B00137: ;
    rdfs:comment "126  Incorporation with Part 3 of Schedule 22 to the Collection Regulations - Abrievated Graph Key: I138"@en-AU ;
    skos:definition "126  Incorporation with Part 3 of Schedule 22 to the Collection Regulations"@en-AU ;
    skos:narrower F1998B00137:105 ;
    skos:prefLabel "Item I138"@en-AU ;
    dcat:accessURL <https://www.legislation.gov.au/F1998B00137/2024-07-06/2024-07-06/text/original/epub/OEBPS/document_1/document_1.html#_Toc171769371> ;
    dcat:landingPage "https://www.legislation.gov.au/F1998B00137/2024-07-06/2024-07-06/text/original/epub/OEBPS/document_1/document_1.html#_Toc171769371"^^xsd:anyURI ;
    dcat:theme legcons:Item .

F1998B00137:139 a legcons:Item,
        owl:Class,
        dcat:Resource ;
    rdfs:label "Item - I139 129  When levy is due for payment Collection Act s 6"@en-AU ;
    dct:isPartOf F1998B00137:105 ;
    dct:isReferencedBy F1998B00137: ;
    rdfs:comment "129  When levy is due for payment Collection Act s 6 - Abrievated Graph Key: I139"@en-AU ;
    skos:definition "129  When levy is due for payment Collection Act s 6"@en-AU ;
    skos:narrower F1998B00137:105 ;
    skos:prefLabel "Item I139"@en-AU ;
    dcat:accessURL <https://www.legislation.gov.au/F1998B00137/2024-07-06/2024-07-06/text/original/epub/OEBPS/document_1/document_1.html#_Toc171769372> ;
    dcat:landingPage "https://www.legislation.gov.au/F1998B00137/2024-07-06/2024-07-06/text/original/epub/OEBPS/document_1/document_1.html#_Toc171769372"^^xsd:anyURI ;
    dcat:theme legcons:Item .

F1998B00137:14 a legcons:Item,
        owl:Class,
        dcat:Resource ;
    rdfs:label "Item - I14 12  Applications for exemptions from giving Secretary quarterly returns"@en-AU ;
    dct:isPartOf F1998B00137:6 ;
    dct:isReferencedBy F1998B00137: ;
    rdfs:comment "12  Applications for exemptions from giving Secretary quarterly returns - Abrievated Graph Key: I14"@en-AU ;
    skos:definition "12  Applications for exemptions from giving Secretary quarterly returns"@en-AU ;
    skos:narrower F1998B00137:6 ;
    skos:prefLabel "Item I14"@en-AU ;
    dcat:accessURL <https://www.legislation.gov.au/F1998B00137/2024-07-06/2024-07-06/text/original/epub/OEBPS/document_1/document_1.html#_Toc171769247> ;
    dcat:landingPage "https://www.legislation.gov.au/F1998B00137/2024-07-06/2024-07-06/text/original/epub/OEBPS/document_1/document_1.html#_Toc171769247"^^xsd:anyURI ;
    dcat:theme legcons:Item .

F1998B00137:140 a legcons:Item,
        owl:Class,
        dcat:Resource ;
    rdfs:label "Item - I140 130  Information in returns under Part 3 of Schedule 22 to the Collection Regulations"@en-AU ;
    dct:isPartOf F1998B00137:105 ;
    dct:isReferencedBy F1998B00137: ;
    rdfs:comment "130  Information in returns under Part 3 of Schedule 22 to the Collection Regulations - Abrievated Graph Key: I140"@en-AU ;
    skos:definition "130  Information in returns under Part 3 of Schedule 22 to the Collection Regulations"@en-AU ;
    skos:narrower F1998B00137:105 ;
    skos:prefLabel "Item I140"@en-AU ;
    dcat:accessURL <https://www.legislation.gov.au/F1998B00137/2024-07-06/2024-07-06/text/original/epub/OEBPS/document_1/document_1.html#_Toc171769373> ;
    dcat:landingPage "https://www.legislation.gov.au/F1998B00137/2024-07-06/2024-07-06/text/original/epub/OEBPS/document_1/document_1.html#_Toc171769373"^^xsd:anyURI ;
    dcat:theme legcons:Item .

F1998B00137:141 a legcons:Item,
        owl:Class,
        dcat:Resource ;
    rdfs:label "Item - I141 131  Information in records under Part 3 of Schedule 22 to the Collection Regulations"@en-AU ;
    dct:isPartOf F1998B00137:105 ;
    dct:isReferencedBy F1998B00137: ;
    rdfs:comment "131  Information in records under Part 3 of Schedule 22 to the Collection Regulations - Abrievated Graph Key: I141"@en-AU ;
    skos:definition "131  Information in records under Part 3 of Schedule 22 to the Collection Regulations"@en-AU ;
    skos:narrower F1998B00137:105 ;
    skos:prefLabel "Item I141"@en-AU ;
    dcat:accessURL <https://www.legislation.gov.au/F1998B00137/2024-07-06/2024-07-06/text/original/epub/OEBPS/document_1/document_1.html#_Toc171769374> ;
    dcat:landingPage "https://www.legislation.gov.au/F1998B00137/2024-07-06/2024-07-06/text/original/epub/OEBPS/document_1/document_1.html#_Toc171769374"^^xsd:anyURI ;
    dcat:theme legcons:Item .

F1998B00137:142 a legcons:Division,
        owl:Class,
        dcat:Resource ;
    rdfs:label "Division - D142 Division 5 Citrus fruits"@en-AU ;
    dct:isPartOf F1998B00137:105 ;
    dct:isReferencedBy F1998B00137: ;
    rdfs:comment "Division 5 Citrus fruits - Abrievated Graph Key: D142"@en-AU ;
    skos:definition "Division 5 Citrus fruits"@en-AU ;
    skos:narrower F1998B00137:105 ;
    skos:prefLabel "Division D142"@en-AU ;
    dcat:accessURL <https://www.legislation.gov.au/F1998B00137/2024-07-06/2024-07-06/text/original/epub/OEBPS/document_1/document_1.html#_Toc171769375> ;
    dcat:landingPage "https://www.legislation.gov.au/F1998B00137/2024-07-06/2024-07-06/text/original/epub/OEBPS/document_1/document_1.html#_Toc171769375"^^xsd:anyURI ;
    dcat:theme legcons:Division .

F1998B00137:143 a legcons:Item,
        owl:Class,
        dcat:Resource ;
    rdfs:label "Item - I143 132  Meaning of expressions for Division"@en-AU ;
    dct:isPartOf F1998B00137:105 ;
    dct:isReferencedBy F1998B00137: ;
    rdfs:comment "132  Meaning of expressions for Division - Abrievated Graph Key: I143"@en-AU ;
    skos:definition "132  Meaning of expressions for Division"@en-AU ;
    skos:narrower F1998B00137:105 ;
    skos:prefLabel "Item I143"@en-AU ;
    dcat:accessURL <https://www.legislation.gov.au/F1998B00137/2024-07-06/2024-07-06/text/original/epub/OEBPS/document_1/document_1.html#_Toc171769376> ;
    dcat:landingPage "https://www.legislation.gov.au/F1998B00137/2024-07-06/2024-07-06/text/original/epub/OEBPS/document_1/document_1.html#_Toc171769376"^^xsd:anyURI ;
    dcat:theme legcons:Item .

F1998B00137:144 a legcons:Item,
        owl:Class,
        dcat:Resource ;
    rdfs:label "Item - I144 133  Incorporation with Part 7 of Schedule 22 to the Collection Regulations"@en-AU ;
    dct:isPartOf F1998B00137:105 ;
    dct:isReferencedBy F1998B00137: ;
    rdfs:comment "133  Incorporation with Part 7 of Schedule 22 to the Collection Regulations - Abrievated Graph Key: I144"@en-AU ;
    skos:definition "133  Incorporation with Part 7 of Schedule 22 to the Collection Regulations"@en-AU ;
    skos:narrower F1998B00137:105 ;
    skos:prefLabel "Item I144"@en-AU ;
    dcat:accessURL <https://www.legislation.gov.au/F1998B00137/2024-07-06/2024-07-06/text/original/epub/OEBPS/document_1/document_1.html#_Toc171769377> ;
    dcat:landingPage "https://www.legislation.gov.au/F1998B00137/2024-07-06/2024-07-06/text/original/epub/OEBPS/document_1/document_1.html#_Toc171769377"^^xsd:anyURI ;
    dcat:theme legcons:Item .

F1998B00137:145 a legcons:Item,
        owl:Class,
        dcat:Resource ;
    rdfs:label "Item - I145 135  When levy is due for payment Collection Act s 6"@en-AU ;
    dct:isPartOf F1998B00137:105 ;
    dct:isReferencedBy F1998B00137: ;
    rdfs:comment "135  When levy is due for payment Collection Act s 6 - Abrievated Graph Key: I145"@en-AU ;
    skos:definition "135  When levy is due for payment Collection Act s 6"@en-AU ;
    skos:narrower F1998B00137:105 ;
    skos:prefLabel "Item I145"@en-AU ;
    dcat:accessURL <https://www.legislation.gov.au/F1998B00137/2024-07-06/2024-07-06/text/original/epub/OEBPS/document_1/document_1.html#_Toc171769378> ;
    dcat:landingPage "https://www.legislation.gov.au/F1998B00137/2024-07-06/2024-07-06/text/original/epub/OEBPS/document_1/document_1.html#_Toc171769378"^^xsd:anyURI ;
    dcat:theme legcons:Item .

F1998B00137:146 a legcons:Item,
        owl:Class,
        dcat:Resource ;
    rdfs:label "Item - I146 136  Information in returns under Part 7 of Schedule 22 to the Collection Regulations"@en-AU ;
    dct:isPartOf F1998B00137:105 ;
    dct:isReferencedBy F1998B00137: ;
    rdfs:comment "136  Information in returns under Part 7 of Schedule 22 to the Collection Regulations - Abrievated Graph Key: I146"@en-AU ;
    skos:definition "136  Information in returns under Part 7 of Schedule 22 to the Collection Regulations"@en-AU ;
    skos:narrower F1998B00137:105 ;
    skos:prefLabel "Item I146"@en-AU ;
    dcat:accessURL <https://www.legislation.gov.au/F1998B00137/2024-07-06/2024-07-06/text/original/epub/OEBPS/document_1/document_1.html#_Toc171769379> ;
    dcat:landingPage "https://www.legislation.gov.au/F1998B00137/2024-07-06/2024-07-06/text/original/epub/OEBPS/document_1/document_1.html#_Toc171769379"^^xsd:anyURI ;
    dcat:theme legcons:Item .

F1998B00137:147 a legcons:Item,
        owl:Class,
        dcat:Resource ;
    rdfs:label "Item - I147 137  Information in records under Part 7 of Schedule 22 to the Collection Regulations"@en-AU ;
    dct:isPartOf F1998B00137:105 ;
    dct:isReferencedBy F1998B00137: ;
    rdfs:comment "137  Information in records under Part 7 of Schedule 22 to the Collection Regulations - Abrievated Graph Key: I147"@en-AU ;
    skos:definition "137  Information in records under Part 7 of Schedule 22 to the Collection Regulations"@en-AU ;
    skos:narrower F1998B00137:105 ;
    skos:prefLabel "Item I147"@en-AU ;
    dcat:accessURL <https://www.legislation.gov.au/F1998B00137/2024-07-06/2024-07-06/text/original/epub/OEBPS/document_1/document_1.html#_Toc171769380> ;
    dcat:landingPage "https://www.legislation.gov.au/F1998B00137/2024-07-06/2024-07-06/text/original/epub/OEBPS/document_1/document_1.html#_Toc171769380"^^xsd:anyURI ;
    dcat:theme legcons:Item .

F1998B00137:148 a legcons:Division,
        owl:Class,
        dcat:Resource ;
    rdfs:label "Division - D148 Division 6 Table grapes"@en-AU ;
    dct:isPartOf F1998B00137:105 ;
    dct:isReferencedBy F1998B00137: ;
    rdfs:comment "Division 6 Table grapes - Abrievated Graph Key: D148"@en-AU ;
    skos:definition "Division 6 Table grapes"@en-AU ;
    skos:narrower F1998B00137:105 ;
    skos:prefLabel "Division D148"@en-AU ;
    dcat:accessURL <https://www.legislation.gov.au/F1998B00137/2024-07-06/2024-07-06/text/original/epub/OEBPS/document_1/document_1.html#_Toc171769381> ;
    dcat:landingPage "https://www.legislation.gov.au/F1998B00137/2024-07-06/2024-07-06/text/original/epub/OEBPS/document_1/document_1.html#_Toc171769381"^^xsd:anyURI ;
    dcat:theme legcons:Division .

F1998B00137:149 a legcons:Item,
        owl:Class,
        dcat:Resource ;
    rdfs:label "Item - I149 138  Meaning of expressions for Division"@en-AU ;
    dct:isPartOf F1998B00137:105 ;
    dct:isReferencedBy F1998B00137: ;
    rdfs:comment "138  Meaning of expressions for Division - Abrievated Graph Key: I149"@en-AU ;
    skos:definition "138  Meaning of expressions for Division"@en-AU ;
    skos:narrower F1998B00137:105 ;
    skos:prefLabel "Item I149"@en-AU ;
    dcat:accessURL <https://www.legislation.gov.au/F1998B00137/2024-07-06/2024-07-06/text/original/epub/OEBPS/document_1/document_1.html#_Toc171769382> ;
    dcat:landingPage "https://www.legislation.gov.au/F1998B00137/2024-07-06/2024-07-06/text/original/epub/OEBPS/document_1/document_1.html#_Toc171769382"^^xsd:anyURI ;
    dcat:theme legcons:Item .

F1998B00137:15 a legcons:Item,
        owl:Class,
        dcat:Resource ;
    rdfs:label "Item - I15 13  How to apply for exemption"@en-AU ;
    dct:isPartOf F1998B00137:6 ;
    dct:isReferencedBy F1998B00137: ;
    rdfs:comment "13  How to apply for exemption - Abrievated Graph Key: I15"@en-AU ;
    skos:definition "13  How to apply for exemption"@en-AU ;
    skos:narrower F1998B00137:6 ;
    skos:prefLabel "Item I15"@en-AU ;
    dcat:accessURL <https://www.legislation.gov.au/F1998B00137/2024-07-06/2024-07-06/text/original/epub/OEBPS/document_1/document_1.html#_Toc171769248> ;
    dcat:landingPage "https://www.legislation.gov.au/F1998B00137/2024-07-06/2024-07-06/text/original/epub/OEBPS/document_1/document_1.html#_Toc171769248"^^xsd:anyURI ;
    dcat:theme legcons:Item .

F1998B00137:150 a legcons:Item,
        owl:Class,
        dcat:Resource ;
    rdfs:label "Item - I150 139  Incorporation with Schedule 20 to the Collection Regulations"@en-AU ;
    dct:isPartOf F1998B00137:105 ;
    dct:isReferencedBy F1998B00137: ;
    rdfs:comment "139  Incorporation with Schedule 20 to the Collection Regulations - Abrievated Graph Key: I150"@en-AU ;
    skos:definition "139  Incorporation with Schedule 20 to the Collection Regulations"@en-AU ;
    skos:narrower F1998B00137:105 ;
    skos:prefLabel "Item I150"@en-AU ;
    dcat:accessURL <https://www.legislation.gov.au/F1998B00137/2024-07-06/2024-07-06/text/original/epub/OEBPS/document_1/document_1.html#_Toc171769383> ;
    dcat:landingPage "https://www.legislation.gov.au/F1998B00137/2024-07-06/2024-07-06/text/original/epub/OEBPS/document_1/document_1.html#_Toc171769383"^^xsd:anyURI ;
    dcat:theme legcons:Item .

F1998B00137:151 a legcons:Item,
        owl:Class,
        dcat:Resource ;
    rdfs:label "Item - I151 141  When levy is due for payment Collection Act s 6"@en-AU ;
    dct:isPartOf F1998B00137:105 ;
    dct:isReferencedBy F1998B00137: ;
    rdfs:comment "141  When levy is due for payment Collection Act s 6 - Abrievated Graph Key: I151"@en-AU ;
    skos:definition "141  When levy is due for payment Collection Act s 6"@en-AU ;
    skos:narrower F1998B00137:105 ;
    skos:prefLabel "Item I151"@en-AU ;
    dcat:accessURL <https://www.legislation.gov.au/F1998B00137/2024-07-06/2024-07-06/text/original/epub/OEBPS/document_1/document_1.html#_Toc171769384> ;
    dcat:landingPage "https://www.legislation.gov.au/F1998B00137/2024-07-06/2024-07-06/text/original/epub/OEBPS/document_1/document_1.html#_Toc171769384"^^xsd:anyURI ;
    dcat:theme legcons:Item .

F1998B00137:152 a legcons:Item,
        owl:Class,
        dcat:Resource ;
    rdfs:label "Item - I152 142  Information in returns under Schedule 20 to the Collection Regulations"@en-AU ;
    dct:isPartOf F1998B00137:105 ;
    dct:isReferencedBy F1998B00137: ;
    rdfs:comment "142  Information in returns under Schedule 20 to the Collection Regulations - Abrievated Graph Key: I152"@en-AU ;
    skos:definition "142  Information in returns under Schedule 20 to the Collection Regulations"@en-AU ;
    skos:narrower F1998B00137:105 ;
    skos:prefLabel "Item I152"@en-AU ;
    dcat:accessURL <https://www.legislation.gov.au/F1998B00137/2024-07-06/2024-07-06/text/original/epub/OEBPS/document_1/document_1.html#_Toc171769385> ;
    dcat:landingPage "https://www.legislation.gov.au/F1998B00137/2024-07-06/2024-07-06/text/original/epub/OEBPS/document_1/document_1.html#_Toc171769385"^^xsd:anyURI ;
    dcat:theme legcons:Item .

F1998B00137:153 a legcons:Item,
        owl:Class,
        dcat:Resource ;
    rdfs:label "Item - I153 143  Information in records under Schedule 20 to the Collection Regulations"@en-AU ;
    dct:isPartOf F1998B00137:105 ;
    dct:isReferencedBy F1998B00137: ;
    rdfs:comment "143  Information in records under Schedule 20 to the Collection Regulations - Abrievated Graph Key: I153"@en-AU ;
    skos:definition "143  Information in records under Schedule 20 to the Collection Regulations"@en-AU ;
    skos:narrower F1998B00137:105 ;
    skos:prefLabel "Item I153"@en-AU ;
    dcat:accessURL <https://www.legislation.gov.au/F1998B00137/2024-07-06/2024-07-06/text/original/epub/OEBPS/document_1/document_1.html#_Toc171769386> ;
    dcat:landingPage "https://www.legislation.gov.au/F1998B00137/2024-07-06/2024-07-06/text/original/epub/OEBPS/document_1/document_1.html#_Toc171769386"^^xsd:anyURI ;
    dcat:theme legcons:Item .

F1998B00137:154 a legcons:Division,
        owl:Class,
        dcat:Resource ;
    rdfs:label "Division - D154 Division 7 Stone fruit"@en-AU ;
    dct:isPartOf F1998B00137:105 ;
    dct:isReferencedBy F1998B00137: ;
    rdfs:comment "Division 7 Stone fruit - Abrievated Graph Key: D154"@en-AU ;
    skos:definition "Division 7 Stone fruit"@en-AU ;
    skos:narrower F1998B00137:105 ;
    skos:prefLabel "Division D154"@en-AU ;
    dcat:accessURL <https://www.legislation.gov.au/F1998B00137/2024-07-06/2024-07-06/text/original/epub/OEBPS/document_1/document_1.html#_Toc171769387> ;
    dcat:landingPage "https://www.legislation.gov.au/F1998B00137/2024-07-06/2024-07-06/text/original/epub/OEBPS/document_1/document_1.html#_Toc171769387"^^xsd:anyURI ;
    dcat:theme legcons:Division .

F1998B00137:155 a legcons:Item,
        owl:Class,
        dcat:Resource ;
    rdfs:label "Item - I155 144  Meaning of expressions for Division"@en-AU ;
    dct:isPartOf F1998B00137:105 ;
    dct:isReferencedBy F1998B00137: ;
    rdfs:comment "144  Meaning of expressions for Division - Abrievated Graph Key: I155"@en-AU ;
    skos:definition "144  Meaning of expressions for Division"@en-AU ;
    skos:narrower F1998B00137:105 ;
    skos:prefLabel "Item I155"@en-AU ;
    dcat:accessURL <https://www.legislation.gov.au/F1998B00137/2024-07-06/2024-07-06/text/original/epub/OEBPS/document_1/document_1.html#_Toc171769388> ;
    dcat:landingPage "https://www.legislation.gov.au/F1998B00137/2024-07-06/2024-07-06/text/original/epub/OEBPS/document_1/document_1.html#_Toc171769388"^^xsd:anyURI ;
    dcat:theme legcons:Item .

F1998B00137:156 a legcons:Item,
        owl:Class,
        dcat:Resource ;
    rdfs:label "Item - I156 145  Incorporation with Part 15 of Schedule 22 to the Collection Regulations"@en-AU ;
    dct:isPartOf F1998B00137:105 ;
    dct:isReferencedBy F1998B00137: ;
    rdfs:comment "145  Incorporation with Part 15 of Schedule 22 to the Collection Regulations - Abrievated Graph Key: I156"@en-AU ;
    skos:definition "145  Incorporation with Part 15 of Schedule 22 to the Collection Regulations"@en-AU ;
    skos:narrower F1998B00137:105 ;
    skos:prefLabel "Item I156"@en-AU ;
    dcat:accessURL <https://www.legislation.gov.au/F1998B00137/2024-07-06/2024-07-06/text/original/epub/OEBPS/document_1/document_1.html#_Toc171769389> ;
    dcat:landingPage "https://www.legislation.gov.au/F1998B00137/2024-07-06/2024-07-06/text/original/epub/OEBPS/document_1/document_1.html#_Toc171769389"^^xsd:anyURI ;
    dcat:theme legcons:Item .

F1998B00137:157 a legcons:Item,
        owl:Class,
        dcat:Resource ;
    rdfs:label "Item - I157 147  When levy is due for payment Collection Act s 6"@en-AU ;
    dct:isPartOf F1998B00137:105 ;
    dct:isReferencedBy F1998B00137: ;
    rdfs:comment "147  When levy is due for payment Collection Act s 6 - Abrievated Graph Key: I157"@en-AU ;
    skos:definition "147  When levy is due for payment Collection Act s 6"@en-AU ;
    skos:narrower F1998B00137:105 ;
    skos:prefLabel "Item I157"@en-AU ;
    dcat:accessURL <https://www.legislation.gov.au/F1998B00137/2024-07-06/2024-07-06/text/original/epub/OEBPS/document_1/document_1.html#_Toc171769390> ;
    dcat:landingPage "https://www.legislation.gov.au/F1998B00137/2024-07-06/2024-07-06/text/original/epub/OEBPS/document_1/document_1.html#_Toc171769390"^^xsd:anyURI ;
    dcat:theme legcons:Item .

F1998B00137:158 a legcons:Item,
        owl:Class,
        dcat:Resource ;
    rdfs:label "Item - I158 148  Information in returns under Part 15 of Schedule 22 to the Collection Regulations"@en-AU ;
    dct:isPartOf F1998B00137:105 ;
    dct:isReferencedBy F1998B00137: ;
    rdfs:comment "148  Information in returns under Part 15 of Schedule 22 to the Collection Regulations - Abrievated Graph Key: I158"@en-AU ;
    skos:definition "148  Information in returns under Part 15 of Schedule 22 to the Collection Regulations"@en-AU ;
    skos:narrower F1998B00137:105 ;
    skos:prefLabel "Item I158"@en-AU ;
    dcat:accessURL <https://www.legislation.gov.au/F1998B00137/2024-07-06/2024-07-06/text/original/epub/OEBPS/document_1/document_1.html#_Toc171769391> ;
    dcat:landingPage "https://www.legislation.gov.au/F1998B00137/2024-07-06/2024-07-06/text/original/epub/OEBPS/document_1/document_1.html#_Toc171769391"^^xsd:anyURI ;
    dcat:theme legcons:Item .

F1998B00137:159 a legcons:Item,
        owl:Class,
        dcat:Resource ;
    rdfs:label "Item - I159 149  Information in records under Part 15 of Schedule 22 to the Collection Regulations"@en-AU ;
    dct:isPartOf F1998B00137:105 ;
    dct:isReferencedBy F1998B00137: ;
    rdfs:comment "149  Information in records under Part 15 of Schedule 22 to the Collection Regulations - Abrievated Graph Key: I159"@en-AU ;
    skos:definition "149  Information in records under Part 15 of Schedule 22 to the Collection Regulations"@en-AU ;
    skos:narrower F1998B00137:105 ;
    skos:prefLabel "Item I159"@en-AU ;
    dcat:accessURL <https://www.legislation.gov.au/F1998B00137/2024-07-06/2024-07-06/text/original/epub/OEBPS/document_1/document_1.html#_Toc171769392> ;
    dcat:landingPage "https://www.legislation.gov.au/F1998B00137/2024-07-06/2024-07-06/text/original/epub/OEBPS/document_1/document_1.html#_Toc171769392"^^xsd:anyURI ;
    dcat:theme legcons:Item .

F1998B00137:16 a legcons:Item,
        owl:Class,
        dcat:Resource ;
    rdfs:label "Item - I16 14  Grant or refusal of exemption"@en-AU ;
    dct:isPartOf F1998B00137:6 ;
    dct:isReferencedBy F1998B00137: ;
    rdfs:comment "14  Grant or refusal of exemption - Abrievated Graph Key: I16"@en-AU ;
    skos:definition "14  Grant or refusal of exemption"@en-AU ;
    skos:narrower F1998B00137:6 ;
    skos:prefLabel "Item I16"@en-AU ;
    dcat:accessURL <https://www.legislation.gov.au/F1998B00137/2024-07-06/2024-07-06/text/original/epub/OEBPS/document_1/document_1.html#_Toc171769249> ;
    dcat:landingPage "https://www.legislation.gov.au/F1998B00137/2024-07-06/2024-07-06/text/original/epub/OEBPS/document_1/document_1.html#_Toc171769249"^^xsd:anyURI ;
    dcat:theme legcons:Item .

F1998B00137:160 a legcons:Division,
        owl:Class,
        dcat:Resource ;
    rdfs:label "Division - D160 Division 8 Macadamia nuts"@en-AU ;
    dct:isPartOf F1998B00137:105 ;
    dct:isReferencedBy F1998B00137: ;
    rdfs:comment "Division 8 Macadamia nuts - Abrievated Graph Key: D160"@en-AU ;
    skos:definition "Division 8 Macadamia nuts"@en-AU ;
    skos:narrower F1998B00137:105 ;
    skos:prefLabel "Division D160"@en-AU ;
    dcat:accessURL <https://www.legislation.gov.au/F1998B00137/2024-07-06/2024-07-06/text/original/epub/OEBPS/document_1/document_1.html#_Toc171769393> ;
    dcat:landingPage "https://www.legislation.gov.au/F1998B00137/2024-07-06/2024-07-06/text/original/epub/OEBPS/document_1/document_1.html#_Toc171769393"^^xsd:anyURI ;
    dcat:theme legcons:Division .

F1998B00137:161 a legcons:Item,
        owl:Class,
        dcat:Resource ;
    rdfs:label "Item - I161 150  Meaning of expressions for Division"@en-AU ;
    dct:isPartOf F1998B00137:105 ;
    dct:isReferencedBy F1998B00137: ;
    rdfs:comment "150  Meaning of expressions for Division - Abrievated Graph Key: I161"@en-AU ;
    skos:definition "150  Meaning of expressions for Division"@en-AU ;
    skos:narrower F1998B00137:105 ;
    skos:prefLabel "Item I161"@en-AU ;
    dcat:accessURL <https://www.legislation.gov.au/F1998B00137/2024-07-06/2024-07-06/text/original/epub/OEBPS/document_1/document_1.html#_Toc171769394> ;
    dcat:landingPage "https://www.legislation.gov.au/F1998B00137/2024-07-06/2024-07-06/text/original/epub/OEBPS/document_1/document_1.html#_Toc171769394"^^xsd:anyURI ;
    dcat:theme legcons:Item .

F1998B00137:162 a legcons:Item,
        owl:Class,
        dcat:Resource ;
    rdfs:label "Item - I162 151  Incorporation with Part 10 of Schedule 22 to the Collection Regulations"@en-AU ;
    dct:isPartOf F1998B00137:105 ;
    dct:isReferencedBy F1998B00137: ;
    rdfs:comment "151  Incorporation with Part 10 of Schedule 22 to the Collection Regulations - Abrievated Graph Key: I162"@en-AU ;
    skos:definition "151  Incorporation with Part 10 of Schedule 22 to the Collection Regulations"@en-AU ;
    skos:narrower F1998B00137:105 ;
    skos:prefLabel "Item I162"@en-AU ;
    dcat:accessURL <https://www.legislation.gov.au/F1998B00137/2024-07-06/2024-07-06/text/original/epub/OEBPS/document_1/document_1.html#_Toc171769395> ;
    dcat:landingPage "https://www.legislation.gov.au/F1998B00137/2024-07-06/2024-07-06/text/original/epub/OEBPS/document_1/document_1.html#_Toc171769395"^^xsd:anyURI ;
    dcat:theme legcons:Item .

F1998B00137:163 a legcons:Item,
        owl:Class,
        dcat:Resource ;
    rdfs:label "Item - I163 152  Macadamia nuts to be eligible horticultural product"@en-AU ;
    dct:isPartOf F1998B00137:105 ;
    dct:isReferencedBy F1998B00137: ;
    rdfs:comment "152  Macadamia nuts to be eligible horticultural product - Abrievated Graph Key: I163"@en-AU ;
    skos:definition "152  Macadamia nuts to be eligible horticultural product"@en-AU ;
    skos:narrower F1998B00137:105 ;
    skos:prefLabel "Item I163"@en-AU ;
    dcat:accessURL <https://www.legislation.gov.au/F1998B00137/2024-07-06/2024-07-06/text/original/epub/OEBPS/document_1/document_1.html#_Toc171769396> ;
    dcat:landingPage "https://www.legislation.gov.au/F1998B00137/2024-07-06/2024-07-06/text/original/epub/OEBPS/document_1/document_1.html#_Toc171769396"^^xsd:anyURI ;
    dcat:theme legcons:Item .

F1998B00137:164 a legcons:Item,
        owl:Class,
        dcat:Resource ;
    rdfs:label "Item - I164 153  Exemption from levy"@en-AU ;
    dct:isPartOf F1998B00137:105 ;
    dct:isReferencedBy F1998B00137: ;
    rdfs:comment "153  Exemption from levy - Abrievated Graph Key: I164"@en-AU ;
    skos:definition "153  Exemption from levy"@en-AU ;
    skos:narrower F1998B00137:105 ;
    skos:prefLabel "Item I164"@en-AU ;
    dcat:accessURL <https://www.legislation.gov.au/F1998B00137/2024-07-06/2024-07-06/text/original/epub/OEBPS/document_1/document_1.html#_Toc171769397> ;
    dcat:landingPage "https://www.legislation.gov.au/F1998B00137/2024-07-06/2024-07-06/text/original/epub/OEBPS/document_1/document_1.html#_Toc171769397"^^xsd:anyURI ;
    dcat:theme legcons:Item .

F1998B00137:165 a legcons:Item,
        owl:Class,
        dcat:Resource ;
    rdfs:label "Item - I165 154  Rate of NRS customs levy"@en-AU ;
    dct:isPartOf F1998B00137:105 ;
    dct:isReferencedBy F1998B00137: ;
    rdfs:comment "154  Rate of NRS customs levy - Abrievated Graph Key: I165"@en-AU ;
    skos:definition "154  Rate of NRS customs levy"@en-AU ;
    skos:narrower F1998B00137:105 ;
    skos:prefLabel "Item I165"@en-AU ;
    dcat:accessURL <https://www.legislation.gov.au/F1998B00137/2024-07-06/2024-07-06/text/original/epub/OEBPS/document_1/document_1.html#_Toc171769398> ;
    dcat:landingPage "https://www.legislation.gov.au/F1998B00137/2024-07-06/2024-07-06/text/original/epub/OEBPS/document_1/document_1.html#_Toc171769398"^^xsd:anyURI ;
    dcat:theme legcons:Item .

F1998B00137:166 a legcons:Item,
        owl:Class,
        dcat:Resource ;
    rdfs:label "Item - I166 155  Rate of NRS excise levy"@en-AU ;
    dct:isPartOf F1998B00137:105 ;
    dct:isReferencedBy F1998B00137: ;
    rdfs:comment "155  Rate of NRS excise levy - Abrievated Graph Key: I166"@en-AU ;
    skos:definition "155  Rate of NRS excise levy"@en-AU ;
    skos:narrower F1998B00137:105 ;
    skos:prefLabel "Item I166"@en-AU ;
    dcat:accessURL <https://www.legislation.gov.au/F1998B00137/2024-07-06/2024-07-06/text/original/epub/OEBPS/document_1/document_1.html#_Toc171769399> ;
    dcat:landingPage "https://www.legislation.gov.au/F1998B00137/2024-07-06/2024-07-06/text/original/epub/OEBPS/document_1/document_1.html#_Toc171769399"^^xsd:anyURI ;
    dcat:theme legcons:Item .

F1998B00137:167 a legcons:Item,
        owl:Class,
        dcat:Resource ;
    rdfs:label "Item - I167 156  When levy is due for payment Collection Act s 6"@en-AU ;
    dct:isPartOf F1998B00137:105 ;
    dct:isReferencedBy F1998B00137: ;
    rdfs:comment "156  When levy is due for payment Collection Act s 6 - Abrievated Graph Key: I167"@en-AU ;
    skos:definition "156  When levy is due for payment Collection Act s 6"@en-AU ;
    skos:narrower F1998B00137:105 ;
    skos:prefLabel "Item I167"@en-AU ;
    dcat:accessURL <https://www.legislation.gov.au/F1998B00137/2024-07-06/2024-07-06/text/original/epub/OEBPS/document_1/document_1.html#_Toc171769400> ;
    dcat:landingPage "https://www.legislation.gov.au/F1998B00137/2024-07-06/2024-07-06/text/original/epub/OEBPS/document_1/document_1.html#_Toc171769400"^^xsd:anyURI ;
    dcat:theme legcons:Item .

F1998B00137:168 a legcons:Item,
        owl:Class,
        dcat:Resource ;
    rdfs:label "Item - I168 157  Information in returns under Part 10 of Schedule 22 to the Collection Regulations"@en-AU ;
    dct:isPartOf F1998B00137:105 ;
    dct:isReferencedBy F1998B00137: ;
    rdfs:comment "157  Information in returns under Part 10 of Schedule 22 to the Collection Regulations - Abrievated Graph Key: I168"@en-AU ;
    skos:definition "157  Information in returns under Part 10 of Schedule 22 to the Collection Regulations"@en-AU ;
    skos:narrower F1998B00137:105 ;
    skos:prefLabel "Item I168"@en-AU ;
    dcat:accessURL <https://www.legislation.gov.au/F1998B00137/2024-07-06/2024-07-06/text/original/epub/OEBPS/document_1/document_1.html#_Toc171769401> ;
    dcat:landingPage "https://www.legislation.gov.au/F1998B00137/2024-07-06/2024-07-06/text/original/epub/OEBPS/document_1/document_1.html#_Toc171769401"^^xsd:anyURI ;
    dcat:theme legcons:Item .

F1998B00137:169 a legcons:Item,
        owl:Class,
        dcat:Resource ;
    rdfs:label "Item - I169 158  Information in records under Part 10 of Schedule 22 to the Collection Regulations"@en-AU ;
    dct:isPartOf F1998B00137:105 ;
    dct:isReferencedBy F1998B00137: ;
    rdfs:comment "158  Information in records under Part 10 of Schedule 22 to the Collection Regulations - Abrievated Graph Key: I169"@en-AU ;
    skos:definition "158  Information in records under Part 10 of Schedule 22 to the Collection Regulations"@en-AU ;
    skos:narrower F1998B00137:105 ;
    skos:prefLabel "Item I169"@en-AU ;
    dcat:accessURL <https://www.legislation.gov.au/F1998B00137/2024-07-06/2024-07-06/text/original/epub/OEBPS/document_1/document_1.html#_Toc171769402> ;
    dcat:landingPage "https://www.legislation.gov.au/F1998B00137/2024-07-06/2024-07-06/text/original/epub/OEBPS/document_1/document_1.html#_Toc171769402"^^xsd:anyURI ;
    dcat:theme legcons:Item .

F1998B00137:17 a legcons:Item,
        owl:Class,
        dcat:Resource ;
    rdfs:label "Item - I17 15  Continuation of exemption"@en-AU ;
    dct:isPartOf F1998B00137:6 ;
    dct:isReferencedBy F1998B00137: ;
    rdfs:comment "15  Continuation of exemption - Abrievated Graph Key: I17"@en-AU ;
    skos:definition "15  Continuation of exemption"@en-AU ;
    skos:narrower F1998B00137:6 ;
    skos:prefLabel "Item I17"@en-AU ;
    dcat:accessURL <https://www.legislation.gov.au/F1998B00137/2024-07-06/2024-07-06/text/original/epub/OEBPS/document_1/document_1.html#_Toc171769250> ;
    dcat:landingPage "https://www.legislation.gov.au/F1998B00137/2024-07-06/2024-07-06/text/original/epub/OEBPS/document_1/document_1.html#_Toc171769250"^^xsd:anyURI ;
    dcat:theme legcons:Item .

F1998B00137:171 a legcons:Item,
        owl:Class,
        dcat:Resource ;
    rdfs:label "Item - I171 183  Meaning of expressions for Part"@en-AU ;
    dct:isPartOf F1998B00137:170 ;
    dct:isReferencedBy F1998B00137: ;
    rdfs:comment "183  Meaning of expressions for Part - Abrievated Graph Key: I171"@en-AU ;
    skos:definition "183  Meaning of expressions for Part"@en-AU ;
    skos:narrower F1998B00137:170 ;
    skos:prefLabel "Item I171"@en-AU ;
    dcat:accessURL <https://www.legislation.gov.au/F1998B00137/2024-07-06/2024-07-06/text/original/epub/OEBPS/document_1/document_1.html#_Toc171769404> ;
    dcat:landingPage "https://www.legislation.gov.au/F1998B00137/2024-07-06/2024-07-06/text/original/epub/OEBPS/document_1/document_1.html#_Toc171769404"^^xsd:anyURI ;
    dcat:theme legcons:Item .

F1998B00137:172 a legcons:Item,
        owl:Class,
        dcat:Resource ;
    rdfs:label "Item - I172 184  Incorporation with Schedule 23 to the Collection Regulations"@en-AU ;
    dct:isPartOf F1998B00137:170 ;
    dct:isReferencedBy F1998B00137: ;
    rdfs:comment "184  Incorporation with Schedule 23 to the Collection Regulations - Abrievated Graph Key: I172"@en-AU ;
    skos:definition "184  Incorporation with Schedule 23 to the Collection Regulations"@en-AU ;
    skos:narrower F1998B00137:170 ;
    skos:prefLabel "Item I172"@en-AU ;
    dcat:accessURL <https://www.legislation.gov.au/F1998B00137/2024-07-06/2024-07-06/text/original/epub/OEBPS/document_1/document_1.html#_Toc171769405> ;
    dcat:landingPage "https://www.legislation.gov.au/F1998B00137/2024-07-06/2024-07-06/text/original/epub/OEBPS/document_1/document_1.html#_Toc171769405"^^xsd:anyURI ;
    dcat:theme legcons:Item .

F1998B00137:173 a legcons:Item,
        owl:Class,
        dcat:Resource ;
    rdfs:label "Item - I173 186  When levy is due for payment Collection Act s 6"@en-AU ;
    dct:isPartOf F1998B00137:170 ;
    dct:isReferencedBy F1998B00137: ;
    rdfs:comment "186  When levy is due for payment Collection Act s 6 - Abrievated Graph Key: I173"@en-AU ;
    skos:definition "186  When levy is due for payment Collection Act s 6"@en-AU ;
    skos:narrower F1998B00137:170 ;
    skos:prefLabel "Item I173"@en-AU ;
    dcat:accessURL <https://www.legislation.gov.au/F1998B00137/2024-07-06/2024-07-06/text/original/epub/OEBPS/document_1/document_1.html#_Toc171769406> ;
    dcat:landingPage "https://www.legislation.gov.au/F1998B00137/2024-07-06/2024-07-06/text/original/epub/OEBPS/document_1/document_1.html#_Toc171769406"^^xsd:anyURI ;
    dcat:theme legcons:Item .

F1998B00137:174 a legcons:Item,
        owl:Class,
        dcat:Resource ;
    rdfs:label "Item - I174 187  Information in returns under Schedule 23 to the Collection Regulations"@en-AU ;
    dct:isPartOf F1998B00137:170 ;
    dct:isReferencedBy F1998B00137: ;
    rdfs:comment "187  Information in returns under Schedule 23 to the Collection Regulations - Abrievated Graph Key: I174"@en-AU ;
    skos:definition "187  Information in returns under Schedule 23 to the Collection Regulations"@en-AU ;
    skos:narrower F1998B00137:170 ;
    skos:prefLabel "Item I174"@en-AU ;
    dcat:accessURL <https://www.legislation.gov.au/F1998B00137/2024-07-06/2024-07-06/text/original/epub/OEBPS/document_1/document_1.html#_Toc171769407> ;
    dcat:landingPage "https://www.legislation.gov.au/F1998B00137/2024-07-06/2024-07-06/text/original/epub/OEBPS/document_1/document_1.html#_Toc171769407"^^xsd:anyURI ;
    dcat:theme legcons:Item .

F1998B00137:175 a legcons:Item,
        owl:Class,
        dcat:Resource ;
    rdfs:label "Item - I175 188  Information in records under Schedule 23 to the Collection Regulations"@en-AU ;
    dct:isPartOf F1998B00137:170 ;
    dct:isReferencedBy F1998B00137: ;
    rdfs:comment "188  Information in records under Schedule 23 to the Collection Regulations - Abrievated Graph Key: I175"@en-AU ;
    skos:definition "188  Information in records under Schedule 23 to the Collection Regulations"@en-AU ;
    skos:narrower F1998B00137:170 ;
    skos:prefLabel "Item I175"@en-AU ;
    dcat:accessURL <https://www.legislation.gov.au/F1998B00137/2024-07-06/2024-07-06/text/original/epub/OEBPS/document_1/document_1.html#_Toc171769408> ;
    dcat:landingPage "https://www.legislation.gov.au/F1998B00137/2024-07-06/2024-07-06/text/original/epub/OEBPS/document_1/document_1.html#_Toc171769408"^^xsd:anyURI ;
    dcat:theme legcons:Item .

F1998B00137:178 a legcons:Item,
        owl:Class,
        dcat:Resource ;
    rdfs:label "Item - I178 189  Meaning of expressions for Part"@en-AU ;
    dct:isPartOf F1998B00137:177 ;
    dct:isReferencedBy F1998B00137: ;
    rdfs:comment "189  Meaning of expressions for Part - Abrievated Graph Key: I178"@en-AU ;
    skos:definition "189  Meaning of expressions for Part"@en-AU ;
    skos:narrower F1998B00137:177 ;
    skos:prefLabel "Item I178"@en-AU ;
    dcat:accessURL <https://www.legislation.gov.au/F1998B00137/2024-07-06/2024-07-06/text/original/epub/OEBPS/document_1/document_1.html#_Toc171769411> ;
    dcat:landingPage "https://www.legislation.gov.au/F1998B00137/2024-07-06/2024-07-06/text/original/epub/OEBPS/document_1/document_1.html#_Toc171769411"^^xsd:anyURI ;
    dcat:theme legcons:Item .

F1998B00137:18 a legcons:Item,
        owl:Class,
        dcat:Resource ;
    rdfs:label "Item - I18 16  What Secretary must consider when making decision"@en-AU ;
    dct:isPartOf F1998B00137:6 ;
    dct:isReferencedBy F1998B00137: ;
    rdfs:comment "16  What Secretary must consider when making decision - Abrievated Graph Key: I18"@en-AU ;
    skos:definition "16  What Secretary must consider when making decision"@en-AU ;
    skos:narrower F1998B00137:6 ;
    skos:prefLabel "Item I18"@en-AU ;
    dcat:accessURL <https://www.legislation.gov.au/F1998B00137/2024-07-06/2024-07-06/text/original/epub/OEBPS/document_1/document_1.html#_Toc171769251> ;
    dcat:landingPage "https://www.legislation.gov.au/F1998B00137/2024-07-06/2024-07-06/text/original/epub/OEBPS/document_1/document_1.html#_Toc171769251"^^xsd:anyURI ;
    dcat:theme legcons:Item .

F1998B00137:180 a legcons:Item,
        owl:Class,
        dcat:Resource ;
    rdfs:label "Item - I180 190  Meaning of expressions for Division"@en-AU ;
    dct:isPartOf F1998B00137:179 ;
    dct:isReferencedBy F1998B00137: ;
    rdfs:comment "190  Meaning of expressions for Division - Abrievated Graph Key: I180"@en-AU ;
    skos:definition "190  Meaning of expressions for Division"@en-AU ;
    skos:narrower F1998B00137:179 ;
    skos:prefLabel "Item I180"@en-AU ;
    dcat:accessURL <https://www.legislation.gov.au/F1998B00137/2024-07-06/2024-07-06/text/original/epub/OEBPS/document_1/document_1.html#_Toc171769413> ;
    dcat:landingPage "https://www.legislation.gov.au/F1998B00137/2024-07-06/2024-07-06/text/original/epub/OEBPS/document_1/document_1.html#_Toc171769413"^^xsd:anyURI ;
    dcat:theme legcons:Item .

F1998B00137:181 a legcons:Item,
        owl:Class,
        dcat:Resource ;
    rdfs:label "Item - I181 191  Incorporation with Schedule 4 to the Collection Regulations"@en-AU ;
    dct:isPartOf F1998B00137:179 ;
    dct:isReferencedBy F1998B00137: ;
    rdfs:comment "191  Incorporation with Schedule 4 to the Collection Regulations - Abrievated Graph Key: I181"@en-AU ;
    skos:definition "191  Incorporation with Schedule 4 to the Collection Regulations"@en-AU ;
    skos:narrower F1998B00137:179 ;
    skos:prefLabel "Item I181"@en-AU ;
    dcat:accessURL <https://www.legislation.gov.au/F1998B00137/2024-07-06/2024-07-06/text/original/epub/OEBPS/document_1/document_1.html#_Toc171769414> ;
    dcat:landingPage "https://www.legislation.gov.au/F1998B00137/2024-07-06/2024-07-06/text/original/epub/OEBPS/document_1/document_1.html#_Toc171769414"^^xsd:anyURI ;
    dcat:theme legcons:Item .

F1998B00137:182 a legcons:Item,
        owl:Class,
        dcat:Resource ;
    rdfs:label "Item - I182 193  When levy is due for payment Collection Act s 6"@en-AU ;
    dct:isPartOf F1998B00137:179 ;
    dct:isReferencedBy F1998B00137: ;
    rdfs:comment "193  When levy is due for payment Collection Act s 6 - Abrievated Graph Key: I182"@en-AU ;
    skos:definition "193  When levy is due for payment Collection Act s 6"@en-AU ;
    skos:narrower F1998B00137:179 ;
    skos:prefLabel "Item I182"@en-AU ;
    dcat:accessURL <https://www.legislation.gov.au/F1998B00137/2024-07-06/2024-07-06/text/original/epub/OEBPS/document_1/document_1.html#_Toc171769415> ;
    dcat:landingPage "https://www.legislation.gov.au/F1998B00137/2024-07-06/2024-07-06/text/original/epub/OEBPS/document_1/document_1.html#_Toc171769415"^^xsd:anyURI ;
    dcat:theme legcons:Item .

F1998B00137:183 a legcons:Item,
        owl:Class,
        dcat:Resource ;
    rdfs:label "Item - I183 194  Information in returns under Schedule 4 to the Collection Regulations"@en-AU ;
    dct:isPartOf F1998B00137:179 ;
    dct:isReferencedBy F1998B00137: ;
    rdfs:comment "194  Information in returns under Schedule 4 to the Collection Regulations - Abrievated Graph Key: I183"@en-AU ;
    skos:definition "194  Information in returns under Schedule 4 to the Collection Regulations"@en-AU ;
    skos:narrower F1998B00137:179 ;
    skos:prefLabel "Item I183"@en-AU ;
    dcat:accessURL <https://www.legislation.gov.au/F1998B00137/2024-07-06/2024-07-06/text/original/epub/OEBPS/document_1/document_1.html#_Toc171769416> ;
    dcat:landingPage "https://www.legislation.gov.au/F1998B00137/2024-07-06/2024-07-06/text/original/epub/OEBPS/document_1/document_1.html#_Toc171769416"^^xsd:anyURI ;
    dcat:theme legcons:Item .

F1998B00137:184 a legcons:Item,
        owl:Class,
        dcat:Resource ;
    rdfs:label "Item - I184 195  Information in records under Schedule 4 to the Collection Regulations"@en-AU ;
    dct:isPartOf F1998B00137:179 ;
    dct:isReferencedBy F1998B00137: ;
    rdfs:comment "195  Information in records under Schedule 4 to the Collection Regulations - Abrievated Graph Key: I184"@en-AU ;
    skos:definition "195  Information in records under Schedule 4 to the Collection Regulations"@en-AU ;
    skos:narrower F1998B00137:179 ;
    skos:prefLabel "Item I184"@en-AU ;
    dcat:accessURL <https://www.legislation.gov.au/F1998B00137/2024-07-06/2024-07-06/text/original/epub/OEBPS/document_1/document_1.html#_Toc171769417> ;
    dcat:landingPage "https://www.legislation.gov.au/F1998B00137/2024-07-06/2024-07-06/text/original/epub/OEBPS/document_1/document_1.html#_Toc171769417"^^xsd:anyURI ;
    dcat:theme legcons:Item .

F1998B00137:185 a legcons:Item,
        owl:Class,
        dcat:Resource ;
    rdfs:label "Item - I185 196  Transitionalobligations about returns under the Primary Industries Levies and Charges Collection Buffalo Cattle and Live stock Regulations 1998"@en-AU ;
    dct:isPartOf F1998B00137:179 ;
    dct:isReferencedBy F1998B00137: ;
    rdfs:comment "196  Transitionalobligations about returns under the Primary Industries Levies and Charges Collection Buffalo Cattle and Live stock Regulations 1998 - Abrievated Graph Key: I185"@en-AU ;
    skos:definition "196  Transitionalobligations about returns under the Primary Industries Levies and Charges Collection Buffalo Cattle and Live stock Regulations 1998"@en-AU ;
    skos:narrower F1998B00137:179 ;
    skos:prefLabel "Item I185"@en-AU ;
    dcat:accessURL <https://www.legislation.gov.au/F1998B00137/2024-07-06/2024-07-06/text/original/epub/OEBPS/document_1/document_1.html#_Toc171769418> ;
    dcat:landingPage "https://www.legislation.gov.au/F1998B00137/2024-07-06/2024-07-06/text/original/epub/OEBPS/document_1/document_1.html#_Toc171769418"^^xsd:anyURI ;
    dcat:theme legcons:Item .

F1998B00137:187 a legcons:Item,
        owl:Class,
        dcat:Resource ;
    rdfs:label "Item - I187 197  Meaning of expressions for Division"@en-AU ;
    dct:isPartOf F1998B00137:186 ;
    dct:isReferencedBy F1998B00137: ;
    rdfs:comment "197  Meaning of expressions for Division - Abrievated Graph Key: I187"@en-AU ;
    skos:definition "197  Meaning of expressions for Division"@en-AU ;
    skos:narrower F1998B00137:186 ;
    skos:prefLabel "Item I187"@en-AU ;
    dcat:accessURL <https://www.legislation.gov.au/F1998B00137/2024-07-06/2024-07-06/text/original/epub/OEBPS/document_1/document_1.html#_Toc171769420> ;
    dcat:landingPage "https://www.legislation.gov.au/F1998B00137/2024-07-06/2024-07-06/text/original/epub/OEBPS/document_1/document_1.html#_Toc171769420"^^xsd:anyURI ;
    dcat:theme legcons:Item .

F1998B00137:188 a legcons:Item,
        owl:Class,
        dcat:Resource ;
    rdfs:label "Item - I188 198  Definitions for Schedule 11 to NRS Excise Levy Act"@en-AU ;
    dct:isPartOf F1998B00137:186 ;
    dct:isReferencedBy F1998B00137: ;
    rdfs:comment "198  Definitions for Schedule 11 to NRS Excise Levy Act - Abrievated Graph Key: I188"@en-AU ;
    skos:definition "198  Definitions for Schedule 11 to NRS Excise Levy Act"@en-AU ;
    skos:narrower F1998B00137:186 ;
    skos:prefLabel "Item I188"@en-AU ;
    dcat:accessURL <https://www.legislation.gov.au/F1998B00137/2024-07-06/2024-07-06/text/original/epub/OEBPS/document_1/document_1.html#_Toc171769421> ;
    dcat:landingPage "https://www.legislation.gov.au/F1998B00137/2024-07-06/2024-07-06/text/original/epub/OEBPS/document_1/document_1.html#_Toc171769421"^^xsd:anyURI ;
    dcat:theme legcons:Item .

F1998B00137:189 a legcons:Item,
        owl:Class,
        dcat:Resource ;
    rdfs:label "Item - I189 199  Incorporation with Schedule 12 to the Collection Regulations"@en-AU ;
    dct:isPartOf F1998B00137:186 ;
    dct:isReferencedBy F1998B00137: ;
    rdfs:comment "199  Incorporation with Schedule 12 to the Collection Regulations - Abrievated Graph Key: I189"@en-AU ;
    skos:definition "199  Incorporation with Schedule 12 to the Collection Regulations"@en-AU ;
    skos:narrower F1998B00137:186 ;
    skos:prefLabel "Item I189"@en-AU ;
    dcat:accessURL <https://www.legislation.gov.au/F1998B00137/2024-07-06/2024-07-06/text/original/epub/OEBPS/document_1/document_1.html#_Toc171769422> ;
    dcat:landingPage "https://www.legislation.gov.au/F1998B00137/2024-07-06/2024-07-06/text/original/epub/OEBPS/document_1/document_1.html#_Toc171769422"^^xsd:anyURI ;
    dcat:theme legcons:Item .

F1998B00137:19 a legcons:Item,
        owl:Class,
        dcat:Resource ;
    rdfs:label "Item - I19 17  Who must give Secretary annual return"@en-AU ;
    dct:isPartOf F1998B00137:6 ;
    dct:isReferencedBy F1998B00137: ;
    rdfs:comment "17  Who must give Secretary annual return - Abrievated Graph Key: I19"@en-AU ;
    skos:definition "17  Who must give Secretary annual return"@en-AU ;
    skos:narrower F1998B00137:6 ;
    skos:prefLabel "Item I19"@en-AU ;
    dcat:accessURL <https://www.legislation.gov.au/F1998B00137/2024-07-06/2024-07-06/text/original/epub/OEBPS/document_1/document_1.html#_Toc171769252> ;
    dcat:landingPage "https://www.legislation.gov.au/F1998B00137/2024-07-06/2024-07-06/text/original/epub/OEBPS/document_1/document_1.html#_Toc171769252"^^xsd:anyURI ;
    dcat:theme legcons:Item .

F1998B00137:190 a legcons:Item,
        owl:Class,
        dcat:Resource ;
    rdfs:label "Item - I190 200  Rate of NRS excise levy on deer slaughter"@en-AU ;
    dct:isPartOf F1998B00137:186 ;
    dct:isReferencedBy F1998B00137: ;
    rdfs:comment "200  Rate of NRS excise levy on deer slaughter - Abrievated Graph Key: I190"@en-AU ;
    skos:definition "200  Rate of NRS excise levy on deer slaughter"@en-AU ;
    skos:narrower F1998B00137:186 ;
    skos:prefLabel "Item I190"@en-AU ;
    dcat:accessURL <https://www.legislation.gov.au/F1998B00137/2024-07-06/2024-07-06/text/original/epub/OEBPS/document_1/document_1.html#_Toc171769423> ;
    dcat:landingPage "https://www.legislation.gov.au/F1998B00137/2024-07-06/2024-07-06/text/original/epub/OEBPS/document_1/document_1.html#_Toc171769423"^^xsd:anyURI ;
    dcat:theme legcons:Item .

F1998B00137:191 a legcons:Item,
        owl:Class,
        dcat:Resource ;
    rdfs:label "Item - I191 201  When levy is due for payment Collection Act s 6"@en-AU ;
    dct:isPartOf F1998B00137:186 ;
    dct:isReferencedBy F1998B00137: ;
    rdfs:comment "201  When levy is due for payment Collection Act s 6 - Abrievated Graph Key: I191"@en-AU ;
    skos:definition "201  When levy is due for payment Collection Act s 6"@en-AU ;
    skos:narrower F1998B00137:186 ;
    skos:prefLabel "Item I191"@en-AU ;
    dcat:accessURL <https://www.legislation.gov.au/F1998B00137/2024-07-06/2024-07-06/text/original/epub/OEBPS/document_1/document_1.html#_Toc171769424> ;
    dcat:landingPage "https://www.legislation.gov.au/F1998B00137/2024-07-06/2024-07-06/text/original/epub/OEBPS/document_1/document_1.html#_Toc171769424"^^xsd:anyURI ;
    dcat:theme legcons:Item .

F1998B00137:192 a legcons:Item,
        owl:Class,
        dcat:Resource ;
    rdfs:label "Item - I192 202  Information in returns under Schedule 12 to the Collection Regulations"@en-AU ;
    dct:isPartOf F1998B00137:186 ;
    dct:isReferencedBy F1998B00137: ;
    rdfs:comment "202  Information in returns under Schedule 12 to the Collection Regulations - Abrievated Graph Key: I192"@en-AU ;
    skos:definition "202  Information in returns under Schedule 12 to the Collection Regulations"@en-AU ;
    skos:narrower F1998B00137:186 ;
    skos:prefLabel "Item I192"@en-AU ;
    dcat:accessURL <https://www.legislation.gov.au/F1998B00137/2024-07-06/2024-07-06/text/original/epub/OEBPS/document_1/document_1.html#_Toc171769425> ;
    dcat:landingPage "https://www.legislation.gov.au/F1998B00137/2024-07-06/2024-07-06/text/original/epub/OEBPS/document_1/document_1.html#_Toc171769425"^^xsd:anyURI ;
    dcat:theme legcons:Item .

F1998B00137:193 a legcons:Item,
        owl:Class,
        dcat:Resource ;
    rdfs:label "Item - I193 203  Information in records under Schedule 12 to the Collection Regulations"@en-AU ;
    dct:isPartOf F1998B00137:186 ;
    dct:isReferencedBy F1998B00137: ;
    rdfs:comment "203  Information in records under Schedule 12 to the Collection Regulations - Abrievated Graph Key: I193"@en-AU ;
    skos:definition "203  Information in records under Schedule 12 to the Collection Regulations"@en-AU ;
    skos:narrower F1998B00137:186 ;
    skos:prefLabel "Item I193"@en-AU ;
    dcat:accessURL <https://www.legislation.gov.au/F1998B00137/2024-07-06/2024-07-06/text/original/epub/OEBPS/document_1/document_1.html#_Toc171769426> ;
    dcat:landingPage "https://www.legislation.gov.au/F1998B00137/2024-07-06/2024-07-06/text/original/epub/OEBPS/document_1/document_1.html#_Toc171769426"^^xsd:anyURI ;
    dcat:theme legcons:Item .

F1998B00137:195 a legcons:Item,
        owl:Class,
        dcat:Resource ;
    rdfs:label "Item - I195 204  Meaning of expressions for Division"@en-AU ;
    dct:isPartOf F1998B00137:194 ;
    dct:isReferencedBy F1998B00137: ;
    rdfs:comment "204  Meaning of expressions for Division - Abrievated Graph Key: I195"@en-AU ;
    skos:definition "204  Meaning of expressions for Division"@en-AU ;
    skos:narrower F1998B00137:194 ;
    skos:prefLabel "Item I195"@en-AU ;
    dcat:accessURL <https://www.legislation.gov.au/F1998B00137/2024-07-06/2024-07-06/text/original/epub/OEBPS/document_1/document_1.html#_Toc171769428> ;
    dcat:landingPage "https://www.legislation.gov.au/F1998B00137/2024-07-06/2024-07-06/text/original/epub/OEBPS/document_1/document_1.html#_Toc171769428"^^xsd:anyURI ;
    dcat:theme legcons:Item .

F1998B00137:196 a legcons:Item,
        owl:Class,
        dcat:Resource ;
    rdfs:label "Item - I196 205  Incorporation with Schedule 31 to the Collection Regulations"@en-AU ;
    dct:isPartOf F1998B00137:194 ;
    dct:isReferencedBy F1998B00137: ;
    rdfs:comment "205  Incorporation with Schedule 31 to the Collection Regulations - Abrievated Graph Key: I196"@en-AU ;
    skos:definition "205  Incorporation with Schedule 31 to the Collection Regulations"@en-AU ;
    skos:narrower F1998B00137:194 ;
    skos:prefLabel "Item I196"@en-AU ;
    dcat:accessURL <https://www.legislation.gov.au/F1998B00137/2024-07-06/2024-07-06/text/original/epub/OEBPS/document_1/document_1.html#_Toc171769429> ;
    dcat:landingPage "https://www.legislation.gov.au/F1998B00137/2024-07-06/2024-07-06/text/original/epub/OEBPS/document_1/document_1.html#_Toc171769429"^^xsd:anyURI ;
    dcat:theme legcons:Item .

F1998B00137:197 a legcons:Item,
        owl:Class,
        dcat:Resource ;
    rdfs:label "Item - I197 206  Rate of NRS excise levy on pig slaughter"@en-AU ;
    dct:isPartOf F1998B00137:194 ;
    dct:isReferencedBy F1998B00137: ;
    rdfs:comment "206  Rate of NRS excise levy on pig slaughter - Abrievated Graph Key: I197"@en-AU ;
    skos:definition "206  Rate of NRS excise levy on pig slaughter"@en-AU ;
    skos:narrower F1998B00137:194 ;
    skos:prefLabel "Item I197"@en-AU ;
    dcat:accessURL <https://www.legislation.gov.au/F1998B00137/2024-07-06/2024-07-06/text/original/epub/OEBPS/document_1/document_1.html#_Toc171769430> ;
    dcat:landingPage "https://www.legislation.gov.au/F1998B00137/2024-07-06/2024-07-06/text/original/epub/OEBPS/document_1/document_1.html#_Toc171769430"^^xsd:anyURI ;
    dcat:theme legcons:Item .

F1998B00137:198 a legcons:Item,
        owl:Class,
        dcat:Resource ;
    rdfs:label "Item - I198 207  When levy is due for payment Collection Act s 6"@en-AU ;
    dct:isPartOf F1998B00137:194 ;
    dct:isReferencedBy F1998B00137: ;
    rdfs:comment "207  When levy is due for payment Collection Act s 6 - Abrievated Graph Key: I198"@en-AU ;
    skos:definition "207  When levy is due for payment Collection Act s 6"@en-AU ;
    skos:narrower F1998B00137:194 ;
    skos:prefLabel "Item I198"@en-AU ;
    dcat:accessURL <https://www.legislation.gov.au/F1998B00137/2024-07-06/2024-07-06/text/original/epub/OEBPS/document_1/document_1.html#_Toc171769431> ;
    dcat:landingPage "https://www.legislation.gov.au/F1998B00137/2024-07-06/2024-07-06/text/original/epub/OEBPS/document_1/document_1.html#_Toc171769431"^^xsd:anyURI ;
    dcat:theme legcons:Item .

F1998B00137:199 a legcons:Item,
        owl:Class,
        dcat:Resource ;
    rdfs:label "Item - I199 208  Information in returns under Schedule 31 to the Collection Regulations"@en-AU ;
    dct:isPartOf F1998B00137:194 ;
    dct:isReferencedBy F1998B00137: ;
    rdfs:comment "208  Information in returns under Schedule 31 to the Collection Regulations - Abrievated Graph Key: I199"@en-AU ;
    skos:definition "208  Information in returns under Schedule 31 to the Collection Regulations"@en-AU ;
    skos:narrower F1998B00137:194 ;
    skos:prefLabel "Item I199"@en-AU ;
    dcat:accessURL <https://www.legislation.gov.au/F1998B00137/2024-07-06/2024-07-06/text/original/epub/OEBPS/document_1/document_1.html#_Toc171769432> ;
    dcat:landingPage "https://www.legislation.gov.au/F1998B00137/2024-07-06/2024-07-06/text/original/epub/OEBPS/document_1/document_1.html#_Toc171769432"^^xsd:anyURI ;
    dcat:theme legcons:Item .

F1998B00137:2 a legcons:Item,
        owl:Class,
        dcat:Resource ;
    rdfs:label "Item - I2 1  Name of Regulations"@en-AU ;
    dct:isPartOf F1998B00137:1 ;
    dct:isReferencedBy F1998B00137: ;
    rdfs:comment "1  Name of Regulations - Abrievated Graph Key: I2"@en-AU ;
    skos:definition "1  Name of Regulations"@en-AU ;
    skos:narrower F1998B00137:1 ;
    skos:prefLabel "Item I2"@en-AU ;
    dcat:accessURL <https://www.legislation.gov.au/F1998B00137/2024-07-06/2024-07-06/text/original/epub/OEBPS/document_1/document_1.html#_Toc171769235> ;
    dcat:landingPage "https://www.legislation.gov.au/F1998B00137/2024-07-06/2024-07-06/text/original/epub/OEBPS/document_1/document_1.html#_Toc171769235"^^xsd:anyURI ;
    dcat:theme legcons:Item .

F1998B00137:20 a legcons:Item,
        owl:Class,
        dcat:Resource ;
    rdfs:label "Item - I20 18  What must be in return"@en-AU ;
    dct:isPartOf F1998B00137:6 ;
    dct:isReferencedBy F1998B00137: ;
    rdfs:comment "18  What must be in return - Abrievated Graph Key: I20"@en-AU ;
    skos:definition "18  What must be in return"@en-AU ;
    skos:narrower F1998B00137:6 ;
    skos:prefLabel "Item I20"@en-AU ;
    dcat:accessURL <https://www.legislation.gov.au/F1998B00137/2024-07-06/2024-07-06/text/original/epub/OEBPS/document_1/document_1.html#_Toc171769253> ;
    dcat:landingPage "https://www.legislation.gov.au/F1998B00137/2024-07-06/2024-07-06/text/original/epub/OEBPS/document_1/document_1.html#_Toc171769253"^^xsd:anyURI ;
    dcat:theme legcons:Item .

F1998B00137:200 a legcons:Item,
        owl:Class,
        dcat:Resource ;
    rdfs:label "Item - I200 209  Information in records under Schedule 31 to the Collection Regulations"@en-AU ;
    dct:isPartOf F1998B00137:194 ;
    dct:isReferencedBy F1998B00137: ;
    rdfs:comment "209  Information in records under Schedule 31 to the Collection Regulations - Abrievated Graph Key: I200"@en-AU ;
    skos:definition "209  Information in records under Schedule 31 to the Collection Regulations"@en-AU ;
    skos:narrower F1998B00137:194 ;
    skos:prefLabel "Item I200"@en-AU ;
    dcat:accessURL <https://www.legislation.gov.au/F1998B00137/2024-07-06/2024-07-06/text/original/epub/OEBPS/document_1/document_1.html#_Toc171769433> ;
    dcat:landingPage "https://www.legislation.gov.au/F1998B00137/2024-07-06/2024-07-06/text/original/epub/OEBPS/document_1/document_1.html#_Toc171769433"^^xsd:anyURI ;
    dcat:theme legcons:Item .

F1998B00137:202 a legcons:Item,
        owl:Class,
        dcat:Resource ;
    rdfs:label "Item - I202 210  Meaning of expressions for Part"@en-AU ;
    dct:isPartOf F1998B00137:201 ;
    dct:isReferencedBy F1998B00137: ;
    rdfs:comment "210  Meaning of expressions for Part - Abrievated Graph Key: I202"@en-AU ;
    skos:definition "210  Meaning of expressions for Part"@en-AU ;
    skos:narrower F1998B00137:201 ;
    skos:prefLabel "Item I202"@en-AU ;
    dcat:accessURL <https://www.legislation.gov.au/F1998B00137/2024-07-06/2024-07-06/text/original/epub/OEBPS/document_1/document_1.html#_Toc171769435> ;
    dcat:landingPage "https://www.legislation.gov.au/F1998B00137/2024-07-06/2024-07-06/text/original/epub/OEBPS/document_1/document_1.html#_Toc171769435"^^xsd:anyURI ;
    dcat:theme legcons:Item .

F1998B00137:203 a legcons:Item,
        owl:Class,
        dcat:Resource ;
    rdfs:label "Item - I203 211  Incorporation with Schedule 28 to the Collection Regulations"@en-AU ;
    dct:isPartOf F1998B00137:201 ;
    dct:isReferencedBy F1998B00137: ;
    rdfs:comment "211  Incorporation with Schedule 28 to the Collection Regulations - Abrievated Graph Key: I203"@en-AU ;
    skos:definition "211  Incorporation with Schedule 28 to the Collection Regulations"@en-AU ;
    skos:narrower F1998B00137:201 ;
    skos:prefLabel "Item I203"@en-AU ;
    dcat:accessURL <https://www.legislation.gov.au/F1998B00137/2024-07-06/2024-07-06/text/original/epub/OEBPS/document_1/document_1.html#_Toc171769436> ;
    dcat:landingPage "https://www.legislation.gov.au/F1998B00137/2024-07-06/2024-07-06/text/original/epub/OEBPS/document_1/document_1.html#_Toc171769436"^^xsd:anyURI ;
    dcat:theme legcons:Item .

F1998B00137:204 a legcons:Item,
        owl:Class,
        dcat:Resource ;
    rdfs:label "Item - I204 213  When levy is due for payment Collection Act s 6"@en-AU ;
    dct:isPartOf F1998B00137:201 ;
    dct:isReferencedBy F1998B00137: ;
    rdfs:comment "213  When levy is due for payment Collection Act s 6 - Abrievated Graph Key: I204"@en-AU ;
    skos:definition "213  When levy is due for payment Collection Act s 6"@en-AU ;
    skos:narrower F1998B00137:201 ;
    skos:prefLabel "Item I204"@en-AU ;
    dcat:accessURL <https://www.legislation.gov.au/F1998B00137/2024-07-06/2024-07-06/text/original/epub/OEBPS/document_1/document_1.html#_Toc171769437> ;
    dcat:landingPage "https://www.legislation.gov.au/F1998B00137/2024-07-06/2024-07-06/text/original/epub/OEBPS/document_1/document_1.html#_Toc171769437"^^xsd:anyURI ;
    dcat:theme legcons:Item .

F1998B00137:205 a legcons:Item,
        owl:Class,
        dcat:Resource ;
    rdfs:label "Item - I205 214  Information in returns under Schedule 28 to the Collection Regulations"@en-AU ;
    dct:isPartOf F1998B00137:201 ;
    dct:isReferencedBy F1998B00137: ;
    rdfs:comment "214  Information in returns under Schedule 28 to the Collection Regulations - Abrievated Graph Key: I205"@en-AU ;
    skos:definition "214  Information in returns under Schedule 28 to the Collection Regulations"@en-AU ;
    skos:narrower F1998B00137:201 ;
    skos:prefLabel "Item I205"@en-AU ;
    dcat:accessURL <https://www.legislation.gov.au/F1998B00137/2024-07-06/2024-07-06/text/original/epub/OEBPS/document_1/document_1.html#_Toc171769438> ;
    dcat:landingPage "https://www.legislation.gov.au/F1998B00137/2024-07-06/2024-07-06/text/original/epub/OEBPS/document_1/document_1.html#_Toc171769438"^^xsd:anyURI ;
    dcat:theme legcons:Item .

F1998B00137:206 a legcons:Item,
        owl:Class,
        dcat:Resource ;
    rdfs:label "Item - I206 215  Information in records under Schedule 28 to the Collection Regulations"@en-AU ;
    dct:isPartOf F1998B00137:201 ;
    dct:isReferencedBy F1998B00137: ;
    rdfs:comment "215  Information in records under Schedule 28 to the Collection Regulations - Abrievated Graph Key: I206"@en-AU ;
    skos:definition "215  Information in records under Schedule 28 to the Collection Regulations"@en-AU ;
    skos:narrower F1998B00137:201 ;
    skos:prefLabel "Item I206"@en-AU ;
    dcat:accessURL <https://www.legislation.gov.au/F1998B00137/2024-07-06/2024-07-06/text/original/epub/OEBPS/document_1/document_1.html#_Toc171769439> ;
    dcat:landingPage "https://www.legislation.gov.au/F1998B00137/2024-07-06/2024-07-06/text/original/epub/OEBPS/document_1/document_1.html#_Toc171769439"^^xsd:anyURI ;
    dcat:theme legcons:Item .

F1998B00137:208 a legcons:Item,
        owl:Class,
        dcat:Resource ;
    rdfs:label "Item - I208 216  Meaning of expressions for Part"@en-AU ;
    dct:isPartOf F1998B00137:207 ;
    dct:isReferencedBy F1998B00137: ;
    rdfs:comment "216  Meaning of expressions for Part - Abrievated Graph Key: I208"@en-AU ;
    skos:definition "216  Meaning of expressions for Part"@en-AU ;
    skos:narrower F1998B00137:207 ;
    skos:prefLabel "Item I208"@en-AU ;
    dcat:accessURL <https://www.legislation.gov.au/F1998B00137/2024-07-06/2024-07-06/text/original/epub/OEBPS/document_1/document_1.html#_Toc171769441> ;
    dcat:landingPage "https://www.legislation.gov.au/F1998B00137/2024-07-06/2024-07-06/text/original/epub/OEBPS/document_1/document_1.html#_Toc171769441"^^xsd:anyURI ;
    dcat:theme legcons:Item .

F1998B00137:209 a legcons:Item,
        owl:Class,
        dcat:Resource ;
    rdfs:label "Item - I209 216 A  Meaning of eligible oilseeds"@en-AU ;
    dct:isPartOf F1998B00137:207 ;
    dct:isReferencedBy F1998B00137: ;
    rdfs:comment "216 A  Meaning of eligible oilseeds - Abrievated Graph Key: I209"@en-AU ;
    skos:definition "216 A  Meaning of eligible oilseeds"@en-AU ;
    skos:narrower F1998B00137:207 ;
    skos:prefLabel "Item I209"@en-AU ;
    dcat:accessURL <https://www.legislation.gov.au/F1998B00137/2024-07-06/2024-07-06/text/original/epub/OEBPS/document_1/document_1.html#_Toc171769442> ;
    dcat:landingPage "https://www.legislation.gov.au/F1998B00137/2024-07-06/2024-07-06/text/original/epub/OEBPS/document_1/document_1.html#_Toc171769442"^^xsd:anyURI ;
    dcat:theme legcons:Item .

F1998B00137:21 a legcons:Item,
        owl:Class,
        dcat:Resource ;
    rdfs:label "Item - I21 19  When and how quarterly return must be given to Secretary"@en-AU ;
    dct:isPartOf F1998B00137:6 ;
    dct:isReferencedBy F1998B00137: ;
    rdfs:comment "19  When and how quarterly return must be given to Secretary - Abrievated Graph Key: I21"@en-AU ;
    skos:definition "19  When and how quarterly return must be given to Secretary"@en-AU ;
    skos:narrower F1998B00137:6 ;
    skos:prefLabel "Item I21"@en-AU ;
    dcat:accessURL <https://www.legislation.gov.au/F1998B00137/2024-07-06/2024-07-06/text/original/epub/OEBPS/document_1/document_1.html#_Toc171769254> ;
    dcat:landingPage "https://www.legislation.gov.au/F1998B00137/2024-07-06/2024-07-06/text/original/epub/OEBPS/document_1/document_1.html#_Toc171769254"^^xsd:anyURI ;
    dcat:theme legcons:Item .

F1998B00137:210 a legcons:Item,
        owl:Class,
        dcat:Resource ;
    rdfs:label "Item - I210 217  Meaning of value"@en-AU ;
    dct:isPartOf F1998B00137:207 ;
    dct:isReferencedBy F1998B00137: ;
    rdfs:comment "217  Meaning of value - Abrievated Graph Key: I210"@en-AU ;
    skos:definition "217  Meaning of value"@en-AU ;
    skos:narrower F1998B00137:207 ;
    skos:prefLabel "Item I210"@en-AU ;
    dcat:accessURL <https://www.legislation.gov.au/F1998B00137/2024-07-06/2024-07-06/text/original/epub/OEBPS/document_1/document_1.html#_Toc171769443> ;
    dcat:landingPage "https://www.legislation.gov.au/F1998B00137/2024-07-06/2024-07-06/text/original/epub/OEBPS/document_1/document_1.html#_Toc171769443"^^xsd:anyURI ;
    dcat:theme legcons:Item .

F1998B00137:211 a legcons:Item,
        owl:Class,
        dcat:Resource ;
    rdfs:label "Item - I211 218  Incorporation with Schedule 29 to the Collection Regulations"@en-AU ;
    dct:isPartOf F1998B00137:207 ;
    dct:isReferencedBy F1998B00137: ;
    rdfs:comment "218  Incorporation with Schedule 29 to the Collection Regulations - Abrievated Graph Key: I211"@en-AU ;
    skos:definition "218  Incorporation with Schedule 29 to the Collection Regulations"@en-AU ;
    skos:narrower F1998B00137:207 ;
    skos:prefLabel "Item I211"@en-AU ;
    dcat:accessURL <https://www.legislation.gov.au/F1998B00137/2024-07-06/2024-07-06/text/original/epub/OEBPS/document_1/document_1.html#_Toc171769444> ;
    dcat:landingPage "https://www.legislation.gov.au/F1998B00137/2024-07-06/2024-07-06/text/original/epub/OEBPS/document_1/document_1.html#_Toc171769444"^^xsd:anyURI ;
    dcat:theme legcons:Item .

F1998B00137:212 a legcons:Item,
        owl:Class,
        dcat:Resource ;
    rdfs:label "Item - I212 219  Rate of NRS levy for eligible oilseeds"@en-AU ;
    dct:isPartOf F1998B00137:207 ;
    dct:isReferencedBy F1998B00137: ;
    rdfs:comment "219  Rate of NRS levy for eligible oilseeds - Abrievated Graph Key: I212"@en-AU ;
    skos:definition "219  Rate of NRS levy for eligible oilseeds"@en-AU ;
    skos:narrower F1998B00137:207 ;
    skos:prefLabel "Item I212"@en-AU ;
    dcat:accessURL <https://www.legislation.gov.au/F1998B00137/2024-07-06/2024-07-06/text/original/epub/OEBPS/document_1/document_1.html#_Toc171769445> ;
    dcat:landingPage "https://www.legislation.gov.au/F1998B00137/2024-07-06/2024-07-06/text/original/epub/OEBPS/document_1/document_1.html#_Toc171769445"^^xsd:anyURI ;
    dcat:theme legcons:Item .

F1998B00137:213 a legcons:Item,
        owl:Class,
        dcat:Resource ;
    rdfs:label "Item - I213 220  When levy is due for payment Collection Act s 6"@en-AU ;
    dct:isPartOf F1998B00137:207 ;
    dct:isReferencedBy F1998B00137: ;
    rdfs:comment "220  When levy is due for payment Collection Act s 6 - Abrievated Graph Key: I213"@en-AU ;
    skos:definition "220  When levy is due for payment Collection Act s 6"@en-AU ;
    skos:narrower F1998B00137:207 ;
    skos:prefLabel "Item I213"@en-AU ;
    dcat:accessURL <https://www.legislation.gov.au/F1998B00137/2024-07-06/2024-07-06/text/original/epub/OEBPS/document_1/document_1.html#_Toc171769446> ;
    dcat:landingPage "https://www.legislation.gov.au/F1998B00137/2024-07-06/2024-07-06/text/original/epub/OEBPS/document_1/document_1.html#_Toc171769446"^^xsd:anyURI ;
    dcat:theme legcons:Item .

F1998B00137:214 a legcons:Item,
        owl:Class,
        dcat:Resource ;
    rdfs:label "Item - I214 221  Information in returns under Schedule 29 to the Collection Regulations"@en-AU ;
    dct:isPartOf F1998B00137:207 ;
    dct:isReferencedBy F1998B00137: ;
    rdfs:comment "221  Information in returns under Schedule 29 to the Collection Regulations - Abrievated Graph Key: I214"@en-AU ;
    skos:definition "221  Information in returns under Schedule 29 to the Collection Regulations"@en-AU ;
    skos:narrower F1998B00137:207 ;
    skos:prefLabel "Item I214"@en-AU ;
    dcat:accessURL <https://www.legislation.gov.au/F1998B00137/2024-07-06/2024-07-06/text/original/epub/OEBPS/document_1/document_1.html#_Toc171769447> ;
    dcat:landingPage "https://www.legislation.gov.au/F1998B00137/2024-07-06/2024-07-06/text/original/epub/OEBPS/document_1/document_1.html#_Toc171769447"^^xsd:anyURI ;
    dcat:theme legcons:Item .

F1998B00137:215 a legcons:Item,
        owl:Class,
        dcat:Resource ;
    rdfs:label "Item - I215 222  Information in records under Schedule 29 to the Collection Regulations"@en-AU ;
    dct:isPartOf F1998B00137:207 ;
    dct:isReferencedBy F1998B00137: ;
    rdfs:comment "222  Information in records under Schedule 29 to the Collection Regulations - Abrievated Graph Key: I215"@en-AU ;
    skos:definition "222  Information in records under Schedule 29 to the Collection Regulations"@en-AU ;
    skos:narrower F1998B00137:207 ;
    skos:prefLabel "Item I215"@en-AU ;
    dcat:accessURL <https://www.legislation.gov.au/F1998B00137/2024-07-06/2024-07-06/text/original/epub/OEBPS/document_1/document_1.html#_Toc171769448> ;
    dcat:landingPage "https://www.legislation.gov.au/F1998B00137/2024-07-06/2024-07-06/text/original/epub/OEBPS/document_1/document_1.html#_Toc171769448"^^xsd:anyURI ;
    dcat:theme legcons:Item .

F1998B00137:217 a legcons:Item,
        owl:Class,
        dcat:Resource ;
    rdfs:label "Item - I217 223  Meaning of expressions for Part"@en-AU ;
    dct:isPartOf F1998B00137:216 ;
    dct:isReferencedBy F1998B00137: ;
    rdfs:comment "223  Meaning of expressions for Part - Abrievated Graph Key: I217"@en-AU ;
    skos:definition "223  Meaning of expressions for Part"@en-AU ;
    skos:narrower F1998B00137:216 ;
    skos:prefLabel "Item I217"@en-AU ;
    dcat:accessURL <https://www.legislation.gov.au/F1998B00137/2024-07-06/2024-07-06/text/original/epub/OEBPS/document_1/document_1.html#_Toc171769450> ;
    dcat:landingPage "https://www.legislation.gov.au/F1998B00137/2024-07-06/2024-07-06/text/original/epub/OEBPS/document_1/document_1.html#_Toc171769450"^^xsd:anyURI ;
    dcat:theme legcons:Item .

F1998B00137:218 a legcons:Item,
        owl:Class,
        dcat:Resource ;
    rdfs:label "Item - I218 224  Levy year Collection Act s 41 definition of levy year"@en-AU ;
    dct:isPartOf F1998B00137:216 ;
    dct:isReferencedBy F1998B00137: ;
    rdfs:comment "224  Levy year Collection Act s 41 definition of levy year - Abrievated Graph Key: I218"@en-AU ;
    skos:definition "224  Levy year Collection Act s 41 definition of levy year"@en-AU ;
    skos:narrower F1998B00137:216 ;
    skos:prefLabel "Item I218"@en-AU ;
    dcat:accessURL <https://www.legislation.gov.au/F1998B00137/2024-07-06/2024-07-06/text/original/epub/OEBPS/document_1/document_1.html#_Toc171769451> ;
    dcat:landingPage "https://www.legislation.gov.au/F1998B00137/2024-07-06/2024-07-06/text/original/epub/OEBPS/document_1/document_1.html#_Toc171769451"^^xsd:anyURI ;
    dcat:theme legcons:Item .

F1998B00137:219 a legcons:Item,
        owl:Class,
        dcat:Resource ;
    rdfs:label "Item - I219 225  Producer and proprietor of processing establishment etc are processor for Collection Act"@en-AU ;
    dct:isPartOf F1998B00137:216 ;
    dct:isReferencedBy F1998B00137: ;
    rdfs:comment "225  Producer and proprietor of processing establishment etc are processor for Collection Act - Abrievated Graph Key: I219"@en-AU ;
    skos:definition "225  Producer and proprietor of processing establishment etc are processor for Collection Act"@en-AU ;
    skos:narrower F1998B00137:216 ;
    skos:prefLabel "Item I219"@en-AU ;
    dcat:accessURL <https://www.legislation.gov.au/F1998B00137/2024-07-06/2024-07-06/text/original/epub/OEBPS/document_1/document_1.html#_Toc171769452> ;
    dcat:landingPage "https://www.legislation.gov.au/F1998B00137/2024-07-06/2024-07-06/text/original/epub/OEBPS/document_1/document_1.html#_Toc171769452"^^xsd:anyURI ;
    dcat:theme legcons:Item .

F1998B00137:22 a legcons:Item,
        owl:Class,
        dcat:Resource ;
    rdfs:label "Item - I22 20  When and how annual return must be given to Secretary"@en-AU ;
    dct:isPartOf F1998B00137:6 ;
    dct:isReferencedBy F1998B00137: ;
    rdfs:comment "20  When and how annual return must be given to Secretary - Abrievated Graph Key: I22"@en-AU ;
    skos:definition "20  When and how annual return must be given to Secretary"@en-AU ;
    skos:narrower F1998B00137:6 ;
    skos:prefLabel "Item I22"@en-AU ;
    dcat:accessURL <https://www.legislation.gov.au/F1998B00137/2024-07-06/2024-07-06/text/original/epub/OEBPS/document_1/document_1.html#_Toc171769255> ;
    dcat:landingPage "https://www.legislation.gov.au/F1998B00137/2024-07-06/2024-07-06/text/original/epub/OEBPS/document_1/document_1.html#_Toc171769255"^^xsd:anyURI ;
    dcat:theme legcons:Item .

F1998B00137:220 a legcons:Item,
        owl:Class,
        dcat:Resource ;
    rdfs:label "Item - I220 226  Owner at time of slaughter is producer for Collection Act"@en-AU ;
    dct:isPartOf F1998B00137:216 ;
    dct:isReferencedBy F1998B00137: ;
    rdfs:comment "226  Owner at time of slaughter is producer for Collection Act - Abrievated Graph Key: I220"@en-AU ;
    skos:definition "226  Owner at time of slaughter is producer for Collection Act"@en-AU ;
    skos:narrower F1998B00137:216 ;
    skos:prefLabel "Item I220"@en-AU ;
    dcat:accessURL <https://www.legislation.gov.au/F1998B00137/2024-07-06/2024-07-06/text/original/epub/OEBPS/document_1/document_1.html#_Toc171769453> ;
    dcat:landingPage "https://www.legislation.gov.au/F1998B00137/2024-07-06/2024-07-06/text/original/epub/OEBPS/document_1/document_1.html#_Toc171769453"^^xsd:anyURI ;
    dcat:theme legcons:Item .

F1998B00137:221 a legcons:Item,
        owl:Class,
        dcat:Resource ;
    rdfs:label "Item - I221 227  Liability of processor as intermediary"@en-AU ;
    dct:isPartOf F1998B00137:216 ;
    dct:isReferencedBy F1998B00137: ;
    rdfs:comment "227  Liability of processor as intermediary - Abrievated Graph Key: I221"@en-AU ;
    skos:definition "227  Liability of processor as intermediary"@en-AU ;
    skos:narrower F1998B00137:216 ;
    skos:prefLabel "Item I221"@en-AU ;
    dcat:accessURL <https://www.legislation.gov.au/F1998B00137/2024-07-06/2024-07-06/text/original/epub/OEBPS/document_1/document_1.html#_Toc171769454> ;
    dcat:landingPage "https://www.legislation.gov.au/F1998B00137/2024-07-06/2024-07-06/text/original/epub/OEBPS/document_1/document_1.html#_Toc171769454"^^xsd:anyURI ;
    dcat:theme legcons:Item .

F1998B00137:222 a legcons:Item,
        owl:Class,
        dcat:Resource ;
    rdfs:label "Item - I222 228  Rate of NRS excise levy on slaughter of ostriches NRS Excise Levy Act Schedule 14 subclause 32"@en-AU ;
    dct:isPartOf F1998B00137:216 ;
    dct:isReferencedBy F1998B00137: ;
    rdfs:comment "228  Rate of NRS excise levy on slaughter of ostriches NRS Excise Levy Act Schedule 14 subclause 32 - Abrievated Graph Key: I222"@en-AU ;
    skos:definition "228  Rate of NRS excise levy on slaughter of ostriches NRS Excise Levy Act Schedule 14 subclause 32"@en-AU ;
    skos:narrower F1998B00137:216 ;
    skos:prefLabel "Item I222"@en-AU ;
    dcat:accessURL <https://www.legislation.gov.au/F1998B00137/2024-07-06/2024-07-06/text/original/epub/OEBPS/document_1/document_1.html#_Toc171769455> ;
    dcat:landingPage "https://www.legislation.gov.au/F1998B00137/2024-07-06/2024-07-06/text/original/epub/OEBPS/document_1/document_1.html#_Toc171769455"^^xsd:anyURI ;
    dcat:theme legcons:Item .

F1998B00137:223 a legcons:Item,
        owl:Class,
        dcat:Resource ;
    rdfs:label "Item - I223 229  Rate of NRS excise levy on slaughter of emus NRS Excise Levy Act Schedule 14 subclause 31"@en-AU ;
    dct:isPartOf F1998B00137:216 ;
    dct:isReferencedBy F1998B00137: ;
    rdfs:comment "229  Rate of NRS excise levy on slaughter of emus NRS Excise Levy Act Schedule 14 subclause 31 - Abrievated Graph Key: I223"@en-AU ;
    skos:definition "229  Rate of NRS excise levy on slaughter of emus NRS Excise Levy Act Schedule 14 subclause 31"@en-AU ;
    skos:narrower F1998B00137:216 ;
    skos:prefLabel "Item I223"@en-AU ;
    dcat:accessURL <https://www.legislation.gov.au/F1998B00137/2024-07-06/2024-07-06/text/original/epub/OEBPS/document_1/document_1.html#_Toc171769456> ;
    dcat:landingPage "https://www.legislation.gov.au/F1998B00137/2024-07-06/2024-07-06/text/original/epub/OEBPS/document_1/document_1.html#_Toc171769456"^^xsd:anyURI ;
    dcat:theme legcons:Item .

F1998B00137:224 a legcons:Item,
        owl:Class,
        dcat:Resource ;
    rdfs:label "Item - I224 230  When levy is due for payment Collection Act s 6"@en-AU ;
    dct:isPartOf F1998B00137:216 ;
    dct:isReferencedBy F1998B00137: ;
    rdfs:comment "230  When levy is due for payment Collection Act s 6 - Abrievated Graph Key: I224"@en-AU ;
    skos:definition "230  When levy is due for payment Collection Act s 6"@en-AU ;
    skos:narrower F1998B00137:216 ;
    skos:prefLabel "Item I224"@en-AU ;
    dcat:accessURL <https://www.legislation.gov.au/F1998B00137/2024-07-06/2024-07-06/text/original/epub/OEBPS/document_1/document_1.html#_Toc171769457> ;
    dcat:landingPage "https://www.legislation.gov.au/F1998B00137/2024-07-06/2024-07-06/text/original/epub/OEBPS/document_1/document_1.html#_Toc171769457"^^xsd:anyURI ;
    dcat:theme legcons:Item .

F1998B00137:225 a legcons:Item,
        owl:Class,
        dcat:Resource ;
    rdfs:label "Item - I225 231  Who must give return to Secretary"@en-AU ;
    dct:isPartOf F1998B00137:216 ;
    dct:isReferencedBy F1998B00137: ;
    rdfs:comment "231  Who must give return to Secretary - Abrievated Graph Key: I225"@en-AU ;
    skos:definition "231  Who must give return to Secretary"@en-AU ;
    skos:narrower F1998B00137:216 ;
    skos:prefLabel "Item I225"@en-AU ;
    dcat:accessURL <https://www.legislation.gov.au/F1998B00137/2024-07-06/2024-07-06/text/original/epub/OEBPS/document_1/document_1.html#_Toc171769458> ;
    dcat:landingPage "https://www.legislation.gov.au/F1998B00137/2024-07-06/2024-07-06/text/original/epub/OEBPS/document_1/document_1.html#_Toc171769458"^^xsd:anyURI ;
    dcat:theme legcons:Item .

F1998B00137:226 a legcons:Item,
        owl:Class,
        dcat:Resource ;
    rdfs:label "Item - I226 232  What must be in return"@en-AU ;
    dct:isPartOf F1998B00137:216 ;
    dct:isReferencedBy F1998B00137: ;
    rdfs:comment "232  What must be in return - Abrievated Graph Key: I226"@en-AU ;
    skos:definition "232  What must be in return"@en-AU ;
    skos:narrower F1998B00137:216 ;
    skos:prefLabel "Item I226"@en-AU ;
    dcat:accessURL <https://www.legislation.gov.au/F1998B00137/2024-07-06/2024-07-06/text/original/epub/OEBPS/document_1/document_1.html#_Toc171769459> ;
    dcat:landingPage "https://www.legislation.gov.au/F1998B00137/2024-07-06/2024-07-06/text/original/epub/OEBPS/document_1/document_1.html#_Toc171769459"^^xsd:anyURI ;
    dcat:theme legcons:Item .

F1998B00137:227 a legcons:Item,
        owl:Class,
        dcat:Resource ;
    rdfs:label "Item - I227 233  When and how return must be given to Secretary"@en-AU ;
    dct:isPartOf F1998B00137:216 ;
    dct:isReferencedBy F1998B00137: ;
    rdfs:comment "233  When and how return must be given to Secretary - Abrievated Graph Key: I227"@en-AU ;
    skos:definition "233  When and how return must be given to Secretary"@en-AU ;
    skos:narrower F1998B00137:216 ;
    skos:prefLabel "Item I227"@en-AU ;
    dcat:accessURL <https://www.legislation.gov.au/F1998B00137/2024-07-06/2024-07-06/text/original/epub/OEBPS/document_1/document_1.html#_Toc171769460> ;
    dcat:landingPage "https://www.legislation.gov.au/F1998B00137/2024-07-06/2024-07-06/text/original/epub/OEBPS/document_1/document_1.html#_Toc171769460"^^xsd:anyURI ;
    dcat:theme legcons:Item .

F1998B00137:228 a legcons:Item,
        owl:Class,
        dcat:Resource ;
    rdfs:label "Item - I228 234  What records must be kept"@en-AU ;
    dct:isPartOf F1998B00137:216 ;
    dct:isReferencedBy F1998B00137: ;
    rdfs:comment "234  What records must be kept - Abrievated Graph Key: I228"@en-AU ;
    skos:definition "234  What records must be kept"@en-AU ;
    skos:narrower F1998B00137:216 ;
    skos:prefLabel "Item I228"@en-AU ;
    dcat:accessURL <https://www.legislation.gov.au/F1998B00137/2024-07-06/2024-07-06/text/original/epub/OEBPS/document_1/document_1.html#_Toc171769461> ;
    dcat:landingPage "https://www.legislation.gov.au/F1998B00137/2024-07-06/2024-07-06/text/original/epub/OEBPS/document_1/document_1.html#_Toc171769461"^^xsd:anyURI ;
    dcat:theme legcons:Item .

F1998B00137:229 a legcons:Item,
        owl:Class,
        dcat:Resource ;
    rdfs:label "Item - I229 235  How long records must be retained"@en-AU ;
    dct:isPartOf F1998B00137:216 ;
    dct:isReferencedBy F1998B00137: ;
    rdfs:comment "235  How long records must be retained - Abrievated Graph Key: I229"@en-AU ;
    skos:definition "235  How long records must be retained"@en-AU ;
    skos:narrower F1998B00137:216 ;
    skos:prefLabel "Item I229"@en-AU ;
    dcat:accessURL <https://www.legislation.gov.au/F1998B00137/2024-07-06/2024-07-06/text/original/epub/OEBPS/document_1/document_1.html#_Toc171769462> ;
    dcat:landingPage "https://www.legislation.gov.au/F1998B00137/2024-07-06/2024-07-06/text/original/epub/OEBPS/document_1/document_1.html#_Toc171769462"^^xsd:anyURI ;
    dcat:theme legcons:Item .

F1998B00137:23 a legcons:Item,
        owl:Class,
        dcat:Resource ;
    rdfs:label "Item - I23 21  What records must be kept"@en-AU ;
    dct:isPartOf F1998B00137:6 ;
    dct:isReferencedBy F1998B00137: ;
    rdfs:comment "21  What records must be kept - Abrievated Graph Key: I23"@en-AU ;
    skos:definition "21  What records must be kept"@en-AU ;
    skos:narrower F1998B00137:6 ;
    skos:prefLabel "Item I23"@en-AU ;
    dcat:accessURL <https://www.legislation.gov.au/F1998B00137/2024-07-06/2024-07-06/text/original/epub/OEBPS/document_1/document_1.html#_Toc171769256> ;
    dcat:landingPage "https://www.legislation.gov.au/F1998B00137/2024-07-06/2024-07-06/text/original/epub/OEBPS/document_1/document_1.html#_Toc171769256"^^xsd:anyURI ;
    dcat:theme legcons:Item .

F1998B00137:230 a legcons:Item,
        owl:Class,
        dcat:Resource ;
    rdfs:label "Item - I230 236  Transitionalobligations about returns under former regulations"@en-AU ;
    dct:isPartOf F1998B00137:216 ;
    dct:isReferencedBy F1998B00137: ;
    rdfs:comment "236  Transitionalobligations about returns under former regulations - Abrievated Graph Key: I230"@en-AU ;
    skos:definition "236  Transitionalobligations about returns under former regulations"@en-AU ;
    skos:narrower F1998B00137:216 ;
    skos:prefLabel "Item I230"@en-AU ;
    dcat:accessURL <https://www.legislation.gov.au/F1998B00137/2024-07-06/2024-07-06/text/original/epub/OEBPS/document_1/document_1.html#_Toc171769463> ;
    dcat:landingPage "https://www.legislation.gov.au/F1998B00137/2024-07-06/2024-07-06/text/original/epub/OEBPS/document_1/document_1.html#_Toc171769463"^^xsd:anyURI ;
    dcat:theme legcons:Item .

F1998B00137:232 a legcons:Item,
        owl:Class,
        dcat:Resource ;
    rdfs:label "Item - I232 237  Meaning of expressions for Part"@en-AU ;
    dct:isPartOf F1998B00137:231 ;
    dct:isReferencedBy F1998B00137: ;
    rdfs:comment "237  Meaning of expressions for Part - Abrievated Graph Key: I232"@en-AU ;
    skos:definition "237  Meaning of expressions for Part"@en-AU ;
    skos:narrower F1998B00137:231 ;
    skos:prefLabel "Item I232"@en-AU ;
    dcat:accessURL <https://www.legislation.gov.au/F1998B00137/2024-07-06/2024-07-06/text/original/epub/OEBPS/document_1/document_1.html#_Toc171769465> ;
    dcat:landingPage "https://www.legislation.gov.au/F1998B00137/2024-07-06/2024-07-06/text/original/epub/OEBPS/document_1/document_1.html#_Toc171769465"^^xsd:anyURI ;
    dcat:theme legcons:Item .

F1998B00137:233 a legcons:Item,
        owl:Class,
        dcat:Resource ;
    rdfs:label "Item - I233 238  Incorporation with Schedules 25 and 27 to the Collection Regulations"@en-AU ;
    dct:isPartOf F1998B00137:231 ;
    dct:isReferencedBy F1998B00137: ;
    rdfs:comment "238  Incorporation with Schedules 25 and 27 to the Collection Regulations - Abrievated Graph Key: I233"@en-AU ;
    skos:definition "238  Incorporation with Schedules 25 and 27 to the Collection Regulations"@en-AU ;
    skos:narrower F1998B00137:231 ;
    skos:prefLabel "Item I233"@en-AU ;
    dcat:accessURL <https://www.legislation.gov.au/F1998B00137/2024-07-06/2024-07-06/text/original/epub/OEBPS/document_1/document_1.html#_Toc171769466> ;
    dcat:landingPage "https://www.legislation.gov.au/F1998B00137/2024-07-06/2024-07-06/text/original/epub/OEBPS/document_1/document_1.html#_Toc171769466"^^xsd:anyURI ;
    dcat:theme legcons:Item .

F1998B00137:234 a legcons:Item,
        owl:Class,
        dcat:Resource ;
    rdfs:label "Item - I234 238 A  Value"@en-AU ;
    dct:isPartOf F1998B00137:231 ;
    dct:isReferencedBy F1998B00137: ;
    rdfs:comment "238 A  Value - Abrievated Graph Key: I234"@en-AU ;
    skos:definition "238 A  Value"@en-AU ;
    skos:narrower F1998B00137:231 ;
    skos:prefLabel "Item I234"@en-AU ;
    dcat:accessURL <https://www.legislation.gov.au/F1998B00137/2024-07-06/2024-07-06/text/original/epub/OEBPS/document_1/document_1.html#_Toc171769467> ;
    dcat:landingPage "https://www.legislation.gov.au/F1998B00137/2024-07-06/2024-07-06/text/original/epub/OEBPS/document_1/document_1.html#_Toc171769467"^^xsd:anyURI ;
    dcat:theme legcons:Item .

F1998B00137:235 a legcons:Item,
        owl:Class,
        dcat:Resource ;
    rdfs:label "Item - I235 239  Rate of NRS customs levy on export of sheep and lambs NRS Customs Levy Act Sch 5 cl 3"@en-AU ;
    dct:isPartOf F1998B00137:231 ;
    dct:isReferencedBy F1998B00137: ;
    rdfs:comment "239  Rate of NRS customs levy on export of sheep and lambs NRS Customs Levy Act Sch 5 cl 3 - Abrievated Graph Key: I235"@en-AU ;
    skos:definition "239  Rate of NRS customs levy on export of sheep and lambs NRS Customs Levy Act Sch 5 cl 3"@en-AU ;
    skos:narrower F1998B00137:231 ;
    skos:prefLabel "Item I235"@en-AU ;
    dcat:accessURL <https://www.legislation.gov.au/F1998B00137/2024-07-06/2024-07-06/text/original/epub/OEBPS/document_1/document_1.html#_Toc171769468> ;
    dcat:landingPage "https://www.legislation.gov.au/F1998B00137/2024-07-06/2024-07-06/text/original/epub/OEBPS/document_1/document_1.html#_Toc171769468"^^xsd:anyURI ;
    dcat:theme legcons:Item .

F1998B00137:236 a legcons:Item,
        owl:Class,
        dcat:Resource ;
    rdfs:label "Item - I236 239 AA  Rate of NRS customs levy on export of goats NRS Customs Levy Act Sch 5 cl 3"@en-AU ;
    dct:isPartOf F1998B00137:231 ;
    dct:isReferencedBy F1998B00137: ;
    rdfs:comment "239 AA  Rate of NRS customs levy on export of goats NRS Customs Levy Act Sch 5 cl 3 - Abrievated Graph Key: I236"@en-AU ;
    skos:definition "239 AA  Rate of NRS customs levy on export of goats NRS Customs Levy Act Sch 5 cl 3"@en-AU ;
    skos:narrower F1998B00137:231 ;
    skos:prefLabel "Item I236"@en-AU ;
    dcat:accessURL <https://www.legislation.gov.au/F1998B00137/2024-07-06/2024-07-06/text/original/epub/OEBPS/document_1/document_1.html#_Toc171769469> ;
    dcat:landingPage "https://www.legislation.gov.au/F1998B00137/2024-07-06/2024-07-06/text/original/epub/OEBPS/document_1/document_1.html#_Toc171769469"^^xsd:anyURI ;
    dcat:theme legcons:Item .

F1998B00137:237 a legcons:Item,
        owl:Class,
        dcat:Resource ;
    rdfs:label "Item - I237 239 A  Sale price"@en-AU ;
    dct:isPartOf F1998B00137:231 ;
    dct:isReferencedBy F1998B00137: ;
    rdfs:comment "239 A  Sale price - Abrievated Graph Key: I237"@en-AU ;
    skos:definition "239 A  Sale price"@en-AU ;
    skos:narrower F1998B00137:231 ;
    skos:prefLabel "Item I237"@en-AU ;
    dcat:accessURL <https://www.legislation.gov.au/F1998B00137/2024-07-06/2024-07-06/text/original/epub/OEBPS/document_1/document_1.html#_Toc171769470> ;
    dcat:landingPage "https://www.legislation.gov.au/F1998B00137/2024-07-06/2024-07-06/text/original/epub/OEBPS/document_1/document_1.html#_Toc171769470"^^xsd:anyURI ;
    dcat:theme legcons:Item .

F1998B00137:238 a legcons:Item,
        owl:Class,
        dcat:Resource ;
    rdfs:label "Item - I238 239 B  When NRS excise levy is not imposed"@en-AU ;
    dct:isPartOf F1998B00137:231 ;
    dct:isReferencedBy F1998B00137: ;
    rdfs:comment "239 B  When NRS excise levy is not imposed - Abrievated Graph Key: I238"@en-AU ;
    skos:definition "239 B  When NRS excise levy is not imposed"@en-AU ;
    skos:narrower F1998B00137:231 ;
    skos:prefLabel "Item I238"@en-AU ;
    dcat:accessURL <https://www.legislation.gov.au/F1998B00137/2024-07-06/2024-07-06/text/original/epub/OEBPS/document_1/document_1.html#_Toc171769471> ;
    dcat:landingPage "https://www.legislation.gov.au/F1998B00137/2024-07-06/2024-07-06/text/original/epub/OEBPS/document_1/document_1.html#_Toc171769471"^^xsd:anyURI ;
    dcat:theme legcons:Item .

F1998B00137:239 a legcons:Item,
        owl:Class,
        dcat:Resource ;
    rdfs:label "Item - I239 240  Rate of NRS excise levy on sheep and lamb sales NRS Excise Levy Act Sch 15 cl 3"@en-AU ;
    dct:isPartOf F1998B00137:231 ;
    dct:isReferencedBy F1998B00137: ;
    rdfs:comment "240  Rate of NRS excise levy on sheep and lamb sales NRS Excise Levy Act Sch 15 cl 3 - Abrievated Graph Key: I239"@en-AU ;
    skos:definition "240  Rate of NRS excise levy on sheep and lamb sales NRS Excise Levy Act Sch 15 cl 3"@en-AU ;
    skos:narrower F1998B00137:231 ;
    skos:prefLabel "Item I239"@en-AU ;
    dcat:accessURL <https://www.legislation.gov.au/F1998B00137/2024-07-06/2024-07-06/text/original/epub/OEBPS/document_1/document_1.html#_Toc171769472> ;
    dcat:landingPage "https://www.legislation.gov.au/F1998B00137/2024-07-06/2024-07-06/text/original/epub/OEBPS/document_1/document_1.html#_Toc171769472"^^xsd:anyURI ;
    dcat:theme legcons:Item .

F1998B00137:24 a legcons:Item,
        owl:Class,
        dcat:Resource ;
    rdfs:label "Item - I24 22  How long records must be retained"@en-AU ;
    dct:isPartOf F1998B00137:6 ;
    dct:isReferencedBy F1998B00137: ;
    rdfs:comment "22  How long records must be retained - Abrievated Graph Key: I24"@en-AU ;
    skos:definition "22  How long records must be retained"@en-AU ;
    skos:narrower F1998B00137:6 ;
    skos:prefLabel "Item I24"@en-AU ;
    dcat:accessURL <https://www.legislation.gov.au/F1998B00137/2024-07-06/2024-07-06/text/original/epub/OEBPS/document_1/document_1.html#_Toc171769257> ;
    dcat:landingPage "https://www.legislation.gov.au/F1998B00137/2024-07-06/2024-07-06/text/original/epub/OEBPS/document_1/document_1.html#_Toc171769257"^^xsd:anyURI ;
    dcat:theme legcons:Item .

F1998B00137:240 a legcons:Item,
        owl:Class,
        dcat:Resource ;
    rdfs:label "Item - I240 241  Rate of NRS excise levy on other sheep and lamb transactions etc NRS Excise Levy Act Sch 15 cl 3"@en-AU ;
    dct:isPartOf F1998B00137:231 ;
    dct:isReferencedBy F1998B00137: ;
    rdfs:comment "241  Rate of NRS excise levy on other sheep and lamb transactions etc NRS Excise Levy Act Sch 15 cl 3 - Abrievated Graph Key: I240"@en-AU ;
    skos:definition "241  Rate of NRS excise levy on other sheep and lamb transactions etc NRS Excise Levy Act Sch 15 cl 3"@en-AU ;
    skos:narrower F1998B00137:231 ;
    skos:prefLabel "Item I240"@en-AU ;
    dcat:accessURL <https://www.legislation.gov.au/F1998B00137/2024-07-06/2024-07-06/text/original/epub/OEBPS/document_1/document_1.html#_Toc171769473> ;
    dcat:landingPage "https://www.legislation.gov.au/F1998B00137/2024-07-06/2024-07-06/text/original/epub/OEBPS/document_1/document_1.html#_Toc171769473"^^xsd:anyURI ;
    dcat:theme legcons:Item .

F1998B00137:241 a legcons:Item,
        owl:Class,
        dcat:Resource ;
    rdfs:label "Item - I241 242  Rate of NRS excise levy on goat transactions NRS Excise Levy Act Sch 15 cl 3"@en-AU ;
    dct:isPartOf F1998B00137:231 ;
    dct:isReferencedBy F1998B00137: ;
    rdfs:comment "242  Rate of NRS excise levy on goat transactions NRS Excise Levy Act Sch 15 cl 3 - Abrievated Graph Key: I241"@en-AU ;
    skos:definition "242  Rate of NRS excise levy on goat transactions NRS Excise Levy Act Sch 15 cl 3"@en-AU ;
    skos:narrower F1998B00137:231 ;
    skos:prefLabel "Item I241"@en-AU ;
    dcat:accessURL <https://www.legislation.gov.au/F1998B00137/2024-07-06/2024-07-06/text/original/epub/OEBPS/document_1/document_1.html#_Toc171769474> ;
    dcat:landingPage "https://www.legislation.gov.au/F1998B00137/2024-07-06/2024-07-06/text/original/epub/OEBPS/document_1/document_1.html#_Toc171769474"^^xsd:anyURI ;
    dcat:theme legcons:Item .

F1998B00137:242 a legcons:Item,
        owl:Class,
        dcat:Resource ;
    rdfs:label "Item - I242 247  When levy is due for payment Collection Act s 6"@en-AU ;
    dct:isPartOf F1998B00137:231 ;
    dct:isReferencedBy F1998B00137: ;
    rdfs:comment "247  When levy is due for payment Collection Act s 6 - Abrievated Graph Key: I242"@en-AU ;
    skos:definition "247  When levy is due for payment Collection Act s 6"@en-AU ;
    skos:narrower F1998B00137:231 ;
    skos:prefLabel "Item I242"@en-AU ;
    dcat:accessURL <https://www.legislation.gov.au/F1998B00137/2024-07-06/2024-07-06/text/original/epub/OEBPS/document_1/document_1.html#_Toc171769475> ;
    dcat:landingPage "https://www.legislation.gov.au/F1998B00137/2024-07-06/2024-07-06/text/original/epub/OEBPS/document_1/document_1.html#_Toc171769475"^^xsd:anyURI ;
    dcat:theme legcons:Item .

F1998B00137:243 a legcons:Item,
        owl:Class,
        dcat:Resource ;
    rdfs:label "Item - I243 248  Information in returns under Schedules 25 and 27 to the Collection Regulations"@en-AU ;
    dct:isPartOf F1998B00137:231 ;
    dct:isReferencedBy F1998B00137: ;
    rdfs:comment "248  Information in returns under Schedules 25 and 27 to the Collection Regulations - Abrievated Graph Key: I243"@en-AU ;
    skos:definition "248  Information in returns under Schedules 25 and 27 to the Collection Regulations"@en-AU ;
    skos:narrower F1998B00137:231 ;
    skos:prefLabel "Item I243"@en-AU ;
    dcat:accessURL <https://www.legislation.gov.au/F1998B00137/2024-07-06/2024-07-06/text/original/epub/OEBPS/document_1/document_1.html#_Toc171769476> ;
    dcat:landingPage "https://www.legislation.gov.au/F1998B00137/2024-07-06/2024-07-06/text/original/epub/OEBPS/document_1/document_1.html#_Toc171769476"^^xsd:anyURI ;
    dcat:theme legcons:Item .

F1998B00137:244 a legcons:Item,
        owl:Class,
        dcat:Resource ;
    rdfs:label "Item - I244 249  Information in records under Schedules 25 and 27 to the Collection Regulations"@en-AU ;
    dct:isPartOf F1998B00137:231 ;
    dct:isReferencedBy F1998B00137: ;
    rdfs:comment "249  Information in records under Schedules 25 and 27 to the Collection Regulations - Abrievated Graph Key: I244"@en-AU ;
    skos:definition "249  Information in records under Schedules 25 and 27 to the Collection Regulations"@en-AU ;
    skos:narrower F1998B00137:231 ;
    skos:prefLabel "Item I244"@en-AU ;
    dcat:accessURL <https://www.legislation.gov.au/F1998B00137/2024-07-06/2024-07-06/text/original/epub/OEBPS/document_1/document_1.html#_Toc171769477> ;
    dcat:landingPage "https://www.legislation.gov.au/F1998B00137/2024-07-06/2024-07-06/text/original/epub/OEBPS/document_1/document_1.html#_Toc171769477"^^xsd:anyURI ;
    dcat:theme legcons:Item .

F1998B00137:245 a legcons:Item,
        owl:Class,
        dcat:Resource ;
    rdfs:label "Item - I245 250  Transitionalobligations about returns under the Primary Industries Levies and Charges Collection Buffalo Cattle and Live stock Regulations 1998"@en-AU ;
    dct:isPartOf F1998B00137:231 ;
    dct:isReferencedBy F1998B00137: ;
    rdfs:comment "250  Transitionalobligations about returns under the Primary Industries Levies and Charges Collection Buffalo Cattle and Live stock Regulations 1998 - Abrievated Graph Key: I245"@en-AU ;
    skos:definition "250  Transitionalobligations about returns under the Primary Industries Levies and Charges Collection Buffalo Cattle and Live stock Regulations 1998"@en-AU ;
    skos:narrower F1998B00137:231 ;
    skos:prefLabel "Item I245"@en-AU ;
    dcat:accessURL <https://www.legislation.gov.au/F1998B00137/2024-07-06/2024-07-06/text/original/epub/OEBPS/document_1/document_1.html#_Toc171769478> ;
    dcat:landingPage "https://www.legislation.gov.au/F1998B00137/2024-07-06/2024-07-06/text/original/epub/OEBPS/document_1/document_1.html#_Toc171769478"^^xsd:anyURI ;
    dcat:theme legcons:Item .

F1998B00137:247 a legcons:Item,
        owl:Class,
        dcat:Resource ;
    rdfs:label "Item - I247 251  Meaning of expressions for Part"@en-AU ;
    dct:isPartOf F1998B00137:246 ;
    dct:isReferencedBy F1998B00137: ;
    rdfs:comment "251  Meaning of expressions for Part - Abrievated Graph Key: I247"@en-AU ;
    skos:definition "251  Meaning of expressions for Part"@en-AU ;
    skos:narrower F1998B00137:246 ;
    skos:prefLabel "Item I247"@en-AU ;
    dcat:accessURL <https://www.legislation.gov.au/F1998B00137/2024-07-06/2024-07-06/text/original/epub/OEBPS/document_1/document_1.html#_Toc171769480> ;
    dcat:landingPage "https://www.legislation.gov.au/F1998B00137/2024-07-06/2024-07-06/text/original/epub/OEBPS/document_1/document_1.html#_Toc171769480"^^xsd:anyURI ;
    dcat:theme legcons:Item .

F1998B00137:248 a legcons:Item,
        owl:Class,
        dcat:Resource ;
    rdfs:label "Item - I248 252  Meaning of value"@en-AU ;
    dct:isPartOf F1998B00137:246 ;
    dct:isReferencedBy F1998B00137: ;
    rdfs:comment "252  Meaning of value - Abrievated Graph Key: I248"@en-AU ;
    skos:definition "252  Meaning of value"@en-AU ;
    skos:narrower F1998B00137:246 ;
    skos:prefLabel "Item I248"@en-AU ;
    dcat:accessURL <https://www.legislation.gov.au/F1998B00137/2024-07-06/2024-07-06/text/original/epub/OEBPS/document_1/document_1.html#_Toc171769481> ;
    dcat:landingPage "https://www.legislation.gov.au/F1998B00137/2024-07-06/2024-07-06/text/original/epub/OEBPS/document_1/document_1.html#_Toc171769481"^^xsd:anyURI ;
    dcat:theme legcons:Item .

F1998B00137:249 a legcons:Item,
        owl:Class,
        dcat:Resource ;
    rdfs:label "Item - I249 253  Incorporation with Schedule 34 to the Collection Regulations"@en-AU ;
    dct:isPartOf F1998B00137:246 ;
    dct:isReferencedBy F1998B00137: ;
    rdfs:comment "253  Incorporation with Schedule 34 to the Collection Regulations - Abrievated Graph Key: I249"@en-AU ;
    skos:definition "253  Incorporation with Schedule 34 to the Collection Regulations"@en-AU ;
    skos:narrower F1998B00137:246 ;
    skos:prefLabel "Item I249"@en-AU ;
    dcat:accessURL <https://www.legislation.gov.au/F1998B00137/2024-07-06/2024-07-06/text/original/epub/OEBPS/document_1/document_1.html#_Toc171769482> ;
    dcat:landingPage "https://www.legislation.gov.au/F1998B00137/2024-07-06/2024-07-06/text/original/epub/OEBPS/document_1/document_1.html#_Toc171769482"^^xsd:anyURI ;
    dcat:theme legcons:Item .

F1998B00137:25 a legcons:Item,
        owl:Class,
        dcat:Resource ;
    rdfs:label "Item - I25 23  Review of decisions"@en-AU ;
    dct:isPartOf F1998B00137:6 ;
    dct:isReferencedBy F1998B00137: ;
    rdfs:comment "23  Review of decisions - Abrievated Graph Key: I25"@en-AU ;
    skos:definition "23  Review of decisions"@en-AU ;
    skos:narrower F1998B00137:6 ;
    skos:prefLabel "Item I25"@en-AU ;
    dcat:accessURL <https://www.legislation.gov.au/F1998B00137/2024-07-06/2024-07-06/text/original/epub/OEBPS/document_1/document_1.html#_Toc171769258> ;
    dcat:landingPage "https://www.legislation.gov.au/F1998B00137/2024-07-06/2024-07-06/text/original/epub/OEBPS/document_1/document_1.html#_Toc171769258"^^xsd:anyURI ;
    dcat:theme legcons:Item .

F1998B00137:250 a legcons:Item,
        owl:Class,
        dcat:Resource ;
    rdfs:label "Item - I250 255  When levy is due for payment Collection Act s 6"@en-AU ;
    dct:isPartOf F1998B00137:246 ;
    dct:isReferencedBy F1998B00137: ;
    rdfs:comment "255  When levy is due for payment Collection Act s 6 - Abrievated Graph Key: I250"@en-AU ;
    skos:definition "255  When levy is due for payment Collection Act s 6"@en-AU ;
    skos:narrower F1998B00137:246 ;
    skos:prefLabel "Item I250"@en-AU ;
    dcat:accessURL <https://www.legislation.gov.au/F1998B00137/2024-07-06/2024-07-06/text/original/epub/OEBPS/document_1/document_1.html#_Toc171769483> ;
    dcat:landingPage "https://www.legislation.gov.au/F1998B00137/2024-07-06/2024-07-06/text/original/epub/OEBPS/document_1/document_1.html#_Toc171769483"^^xsd:anyURI ;
    dcat:theme legcons:Item .

F1998B00137:251 a legcons:Item,
        owl:Class,
        dcat:Resource ;
    rdfs:label "Item - I251 256  Information in returns under Schedule 34 to the Collection Regulations"@en-AU ;
    dct:isPartOf F1998B00137:246 ;
    dct:isReferencedBy F1998B00137: ;
    rdfs:comment "256  Information in returns under Schedule 34 to the Collection Regulations - Abrievated Graph Key: I251"@en-AU ;
    skos:definition "256  Information in returns under Schedule 34 to the Collection Regulations"@en-AU ;
    skos:narrower F1998B00137:246 ;
    skos:prefLabel "Item I251"@en-AU ;
    dcat:accessURL <https://www.legislation.gov.au/F1998B00137/2024-07-06/2024-07-06/text/original/epub/OEBPS/document_1/document_1.html#_Toc171769484> ;
    dcat:landingPage "https://www.legislation.gov.au/F1998B00137/2024-07-06/2024-07-06/text/original/epub/OEBPS/document_1/document_1.html#_Toc171769484"^^xsd:anyURI ;
    dcat:theme legcons:Item .

F1998B00137:252 a legcons:Item,
        owl:Class,
        dcat:Resource ;
    rdfs:label "Item - I252 257  Information in records under Schedule 34 to the Collection Regulations"@en-AU ;
    dct:isPartOf F1998B00137:246 ;
    dct:isReferencedBy F1998B00137: ;
    rdfs:comment "257  Information in records under Schedule 34 to the Collection Regulations - Abrievated Graph Key: I252"@en-AU ;
    skos:definition "257  Information in records under Schedule 34 to the Collection Regulations"@en-AU ;
    skos:narrower F1998B00137:246 ;
    skos:prefLabel "Item I252"@en-AU ;
    dcat:accessURL <https://www.legislation.gov.au/F1998B00137/2024-07-06/2024-07-06/text/original/epub/OEBPS/document_1/document_1.html#_Toc171769485> ;
    dcat:landingPage "https://www.legislation.gov.au/F1998B00137/2024-07-06/2024-07-06/text/original/epub/OEBPS/document_1/document_1.html#_Toc171769485"^^xsd:anyURI ;
    dcat:theme legcons:Item .

F1998B00137:253 a legcons:Schedule,
        owl:Class,
        dcat:Resource ;
    rdfs:label "Schedule - S253 Schedule 1 ALeviable aquatic animals and aquatic animal products"@en-AU ;
    dct:hasPart F1998B00137:254 ;
    dct:isReferencedBy F1998B00137: ;
    rdfs:comment "Schedule 1 ALeviable aquatic animals and aquatic animal products - Abrievated Graph Key: S253"@en-AU ;
    skos:broader F1998B00137:254 ;
    skos:definition "Schedule 1 ALeviable aquatic animals and aquatic animal products"@en-AU ;
    skos:prefLabel "Schedule S253"@en-AU ;
    dcat:accessURL <https://www.legislation.gov.au/F1998B00137/2024-07-06/2024-07-06/text/original/epub/OEBPS/document_1/document_1.html#_Toc171769486> ;
    dcat:landingPage "https://www.legislation.gov.au/F1998B00137/2024-07-06/2024-07-06/text/original/epub/OEBPS/document_1/document_1.html#_Toc171769486"^^xsd:anyURI ;
    dcat:theme legcons:Schedule .

F1998B00137:255 a legcons:Item,
        owl:Class,
        dcat:Resource ;
    rdfs:label "Item - I255 Endnote 1 About the endnotes"@en-AU ;
    dct:isPartOf F1998B00137:254 ;
    dct:isReferencedBy F1998B00137: ;
    rdfs:comment "Endnote 1 About the endnotes - Abrievated Graph Key: I255"@en-AU ;
    skos:definition "Endnote 1 About the endnotes"@en-AU ;
    skos:narrower F1998B00137:254 ;
    skos:prefLabel "Item I255"@en-AU ;
    dcat:accessURL <https://www.legislation.gov.au/F1998B00137/2024-07-06/2024-07-06/text/original/epub/OEBPS/document_1/document_1.html#_Toc171769488> ;
    dcat:landingPage "https://www.legislation.gov.au/F1998B00137/2024-07-06/2024-07-06/text/original/epub/OEBPS/document_1/document_1.html#_Toc171769488"^^xsd:anyURI ;
    dcat:theme legcons:Item .

F1998B00137:256 a legcons:Item,
        owl:Class,
        dcat:Resource ;
    rdfs:label "Item - I256 Endnote 2 Abbreviation key"@en-AU ;
    dct:isPartOf F1998B00137:254 ;
    dct:isReferencedBy F1998B00137: ;
    rdfs:comment "Endnote 2 Abbreviation key - Abrievated Graph Key: I256"@en-AU ;
    skos:definition "Endnote 2 Abbreviation key"@en-AU ;
    skos:narrower F1998B00137:254 ;
    skos:prefLabel "Item I256"@en-AU ;
    dcat:accessURL <https://www.legislation.gov.au/F1998B00137/2024-07-06/2024-07-06/text/original/epub/OEBPS/document_1/document_1.html#_Toc171769489> ;
    dcat:landingPage "https://www.legislation.gov.au/F1998B00137/2024-07-06/2024-07-06/text/original/epub/OEBPS/document_1/document_1.html#_Toc171769489"^^xsd:anyURI ;
    dcat:theme legcons:Item .

F1998B00137:257 a legcons:Item,
        owl:Class,
        dcat:Resource ;
    rdfs:label "Item - I257 Endnote 3 Legislation history"@en-AU ;
    dct:isPartOf F1998B00137:254 ;
    dct:isReferencedBy F1998B00137: ;
    rdfs:comment "Endnote 3 Legislation history - Abrievated Graph Key: I257"@en-AU ;
    skos:definition "Endnote 3 Legislation history"@en-AU ;
    skos:narrower F1998B00137:254 ;
    skos:prefLabel "Item I257"@en-AU ;
    dcat:accessURL <https://www.legislation.gov.au/F1998B00137/2024-07-06/2024-07-06/text/original/epub/OEBPS/document_1/document_1.html#_Toc171769490> ;
    dcat:landingPage "https://www.legislation.gov.au/F1998B00137/2024-07-06/2024-07-06/text/original/epub/OEBPS/document_1/document_1.html#_Toc171769490"^^xsd:anyURI ;
    dcat:theme legcons:Item .

F1998B00137:258 a legcons:Item,
        owl:Class,
        dcat:Resource ;
    rdfs:label "Item - I258 Endnote 4 Amendment history"@en-AU ;
    dct:isPartOf F1998B00137:254 ;
    dct:isReferencedBy F1998B00137: ;
    rdfs:comment "Endnote 4 Amendment history - Abrievated Graph Key: I258"@en-AU ;
    skos:definition "Endnote 4 Amendment history"@en-AU ;
    skos:narrower F1998B00137:254 ;
    skos:prefLabel "Item I258"@en-AU ;
    dcat:accessURL <https://www.legislation.gov.au/F1998B00137/2024-07-06/2024-07-06/text/original/epub/OEBPS/document_1/document_1.html#_Toc171769491> ;
    dcat:landingPage "https://www.legislation.gov.au/F1998B00137/2024-07-06/2024-07-06/text/original/epub/OEBPS/document_1/document_1.html#_Toc171769491"^^xsd:anyURI ;
    dcat:theme legcons:Item .

F1998B00137:26 a legcons:Item,
        owl:Class,
        dcat:Resource ;
    rdfs:label "Item - I26 24  Transitionalobligations about returns under former regulations"@en-AU ;
    dct:isPartOf F1998B00137:6 ;
    dct:isReferencedBy F1998B00137: ;
    rdfs:comment "24  Transitionalobligations about returns under former regulations - Abrievated Graph Key: I26"@en-AU ;
    skos:definition "24  Transitionalobligations about returns under former regulations"@en-AU ;
    skos:narrower F1998B00137:6 ;
    skos:prefLabel "Item I26"@en-AU ;
    dcat:accessURL <https://www.legislation.gov.au/F1998B00137/2024-07-06/2024-07-06/text/original/epub/OEBPS/document_1/document_1.html#_Toc171769259> ;
    dcat:landingPage "https://www.legislation.gov.au/F1998B00137/2024-07-06/2024-07-06/text/original/epub/OEBPS/document_1/document_1.html#_Toc171769259"^^xsd:anyURI ;
    dcat:theme legcons:Item .

F1998B00137:27 a legcons:Item,
        owl:Class,
        dcat:Resource ;
    rdfs:label "Item - I27 24 A  Exempt aquatic animals and aquatic animal products"@en-AU ;
    dct:isPartOf F1998B00137:6 ;
    dct:isReferencedBy F1998B00137: ;
    rdfs:comment "24 A  Exempt aquatic animals and aquatic animal products - Abrievated Graph Key: I27"@en-AU ;
    skos:definition "24 A  Exempt aquatic animals and aquatic animal products"@en-AU ;
    skos:narrower F1998B00137:6 ;
    skos:prefLabel "Item I27"@en-AU ;
    dcat:accessURL <https://www.legislation.gov.au/F1998B00137/2024-07-06/2024-07-06/text/original/epub/OEBPS/document_1/document_1.html#_Toc171769260> ;
    dcat:landingPage "https://www.legislation.gov.au/F1998B00137/2024-07-06/2024-07-06/text/original/epub/OEBPS/document_1/document_1.html#_Toc171769260"^^xsd:anyURI ;
    dcat:theme legcons:Item .

F1998B00137:29 a legcons:Item,
        owl:Class,
        dcat:Resource ;
    rdfs:label "Item - I29 25  Meaning of expressions for Part"@en-AU ;
    dct:isPartOf F1998B00137:28 ;
    dct:isReferencedBy F1998B00137: ;
    rdfs:comment "25  Meaning of expressions for Part - Abrievated Graph Key: I29"@en-AU ;
    skos:definition "25  Meaning of expressions for Part"@en-AU ;
    skos:narrower F1998B00137:28 ;
    skos:prefLabel "Item I29"@en-AU ;
    dcat:accessURL <https://www.legislation.gov.au/F1998B00137/2024-07-06/2024-07-06/text/original/epub/OEBPS/document_1/document_1.html#_Toc171769262> ;
    dcat:landingPage "https://www.legislation.gov.au/F1998B00137/2024-07-06/2024-07-06/text/original/epub/OEBPS/document_1/document_1.html#_Toc171769262"^^xsd:anyURI ;
    dcat:theme legcons:Item .

F1998B00137:3 a legcons:Item,
        owl:Class,
        dcat:Resource ;
    rdfs:label "Item - I3 3  Definitions for Regulations generally"@en-AU ;
    dct:isPartOf F1998B00137:1 ;
    dct:isReferencedBy F1998B00137: ;
    rdfs:comment "3  Definitions for Regulations generally - Abrievated Graph Key: I3"@en-AU ;
    skos:definition "3  Definitions for Regulations generally"@en-AU ;
    skos:narrower F1998B00137:1 ;
    skos:prefLabel "Item I3"@en-AU ;
    dcat:accessURL <https://www.legislation.gov.au/F1998B00137/2024-07-06/2024-07-06/text/original/epub/OEBPS/document_1/document_1.html#_Toc171769236> ;
    dcat:landingPage "https://www.legislation.gov.au/F1998B00137/2024-07-06/2024-07-06/text/original/epub/OEBPS/document_1/document_1.html#_Toc171769236"^^xsd:anyURI ;
    dcat:theme legcons:Item .

F1998B00137:30 a legcons:Item,
        owl:Class,
        dcat:Resource ;
    rdfs:label "Item - I30 26  Incorporation with Schedules 6 and 7 to the Collection Regulations"@en-AU ;
    dct:isPartOf F1998B00137:28 ;
    dct:isReferencedBy F1998B00137: ;
    rdfs:comment "26  Incorporation with Schedules 6 and 7 to the Collection Regulations - Abrievated Graph Key: I30"@en-AU ;
    skos:definition "26  Incorporation with Schedules 6 and 7 to the Collection Regulations"@en-AU ;
    skos:narrower F1998B00137:28 ;
    skos:prefLabel "Item I30"@en-AU ;
    dcat:accessURL <https://www.legislation.gov.au/F1998B00137/2024-07-06/2024-07-06/text/original/epub/OEBPS/document_1/document_1.html#_Toc171769263> ;
    dcat:landingPage "https://www.legislation.gov.au/F1998B00137/2024-07-06/2024-07-06/text/original/epub/OEBPS/document_1/document_1.html#_Toc171769263"^^xsd:anyURI ;
    dcat:theme legcons:Item .

F1998B00137:31 a legcons:Item,
        owl:Class,
        dcat:Resource ;
    rdfs:label "Item - I31 27  When NRS excise levy is not imposed"@en-AU ;
    dct:isPartOf F1998B00137:28 ;
    dct:isReferencedBy F1998B00137: ;
    rdfs:comment "27  When NRS excise levy is not imposed - Abrievated Graph Key: I31"@en-AU ;
    skos:definition "27  When NRS excise levy is not imposed"@en-AU ;
    skos:narrower F1998B00137:28 ;
    skos:prefLabel "Item I31"@en-AU ;
    dcat:accessURL <https://www.legislation.gov.au/F1998B00137/2024-07-06/2024-07-06/text/original/epub/OEBPS/document_1/document_1.html#_Toc171769264> ;
    dcat:landingPage "https://www.legislation.gov.au/F1998B00137/2024-07-06/2024-07-06/text/original/epub/OEBPS/document_1/document_1.html#_Toc171769264"^^xsd:anyURI ;
    dcat:theme legcons:Item .

F1998B00137:32 a legcons:Item,
        owl:Class,
        dcat:Resource ;
    rdfs:label "Item - I32 28  Rate of NRS customs levy"@en-AU ;
    dct:isPartOf F1998B00137:28 ;
    dct:isReferencedBy F1998B00137: ;
    rdfs:comment "28  Rate of NRS customs levy - Abrievated Graph Key: I32"@en-AU ;
    skos:definition "28  Rate of NRS customs levy"@en-AU ;
    skos:narrower F1998B00137:28 ;
    skos:prefLabel "Item I32"@en-AU ;
    dcat:accessURL <https://www.legislation.gov.au/F1998B00137/2024-07-06/2024-07-06/text/original/epub/OEBPS/document_1/document_1.html#_Toc171769265> ;
    dcat:landingPage "https://www.legislation.gov.au/F1998B00137/2024-07-06/2024-07-06/text/original/epub/OEBPS/document_1/document_1.html#_Toc171769265"^^xsd:anyURI ;
    dcat:theme legcons:Item .

F1998B00137:33 a legcons:Item,
        owl:Class,
        dcat:Resource ;
    rdfs:label "Item - I33 28 A  Rate of NRS excise levy"@en-AU ;
    dct:isPartOf F1998B00137:28 ;
    dct:isReferencedBy F1998B00137: ;
    rdfs:comment "28 A  Rate of NRS excise levy - Abrievated Graph Key: I33"@en-AU ;
    skos:definition "28 A  Rate of NRS excise levy"@en-AU ;
    skos:narrower F1998B00137:28 ;
    skos:prefLabel "Item I33"@en-AU ;
    dcat:accessURL <https://www.legislation.gov.au/F1998B00137/2024-07-06/2024-07-06/text/original/epub/OEBPS/document_1/document_1.html#_Toc171769266> ;
    dcat:landingPage "https://www.legislation.gov.au/F1998B00137/2024-07-06/2024-07-06/text/original/epub/OEBPS/document_1/document_1.html#_Toc171769266"^^xsd:anyURI ;
    dcat:theme legcons:Item .

F1998B00137:34 a legcons:Item,
        owl:Class,
        dcat:Resource ;
    rdfs:label "Item - I34 29  When levy is due for payment Collection Act s 6"@en-AU ;
    dct:isPartOf F1998B00137:28 ;
    dct:isReferencedBy F1998B00137: ;
    rdfs:comment "29  When levy is due for payment Collection Act s 6 - Abrievated Graph Key: I34"@en-AU ;
    skos:definition "29  When levy is due for payment Collection Act s 6"@en-AU ;
    skos:narrower F1998B00137:28 ;
    skos:prefLabel "Item I34"@en-AU ;
    dcat:accessURL <https://www.legislation.gov.au/F1998B00137/2024-07-06/2024-07-06/text/original/epub/OEBPS/document_1/document_1.html#_Toc171769267> ;
    dcat:landingPage "https://www.legislation.gov.au/F1998B00137/2024-07-06/2024-07-06/text/original/epub/OEBPS/document_1/document_1.html#_Toc171769267"^^xsd:anyURI ;
    dcat:theme legcons:Item .

F1998B00137:35 a legcons:Item,
        owl:Class,
        dcat:Resource ;
    rdfs:label "Item - I35 30  Information in returns under Schedules 6 and 7 to the Collection Regulations"@en-AU ;
    dct:isPartOf F1998B00137:28 ;
    dct:isReferencedBy F1998B00137: ;
    rdfs:comment "30  Information in returns under Schedules 6 and 7 to the Collection Regulations - Abrievated Graph Key: I35"@en-AU ;
    skos:definition "30  Information in returns under Schedules 6 and 7 to the Collection Regulations"@en-AU ;
    skos:narrower F1998B00137:28 ;
    skos:prefLabel "Item I35"@en-AU ;
    dcat:accessURL <https://www.legislation.gov.au/F1998B00137/2024-07-06/2024-07-06/text/original/epub/OEBPS/document_1/document_1.html#_Toc171769268> ;
    dcat:landingPage "https://www.legislation.gov.au/F1998B00137/2024-07-06/2024-07-06/text/original/epub/OEBPS/document_1/document_1.html#_Toc171769268"^^xsd:anyURI ;
    dcat:theme legcons:Item .

F1998B00137:36 a legcons:Item,
        owl:Class,
        dcat:Resource ;
    rdfs:label "Item - I36 31  Information in records under Schedules 6 and 7 to the Collection Regulations"@en-AU ;
    dct:isPartOf F1998B00137:28 ;
    dct:isReferencedBy F1998B00137: ;
    rdfs:comment "31  Information in records under Schedules 6 and 7 to the Collection Regulations - Abrievated Graph Key: I36"@en-AU ;
    skos:definition "31  Information in records under Schedules 6 and 7 to the Collection Regulations"@en-AU ;
    skos:narrower F1998B00137:28 ;
    skos:prefLabel "Item I36"@en-AU ;
    dcat:accessURL <https://www.legislation.gov.au/F1998B00137/2024-07-06/2024-07-06/text/original/epub/OEBPS/document_1/document_1.html#_Toc171769269> ;
    dcat:landingPage "https://www.legislation.gov.au/F1998B00137/2024-07-06/2024-07-06/text/original/epub/OEBPS/document_1/document_1.html#_Toc171769269"^^xsd:anyURI ;
    dcat:theme legcons:Item .

F1998B00137:37 a legcons:Item,
        owl:Class,
        dcat:Resource ;
    rdfs:label "Item - I37 32  Transitionalobligations about returns under the Primary Industries Levies and Charges Collection Buffalo Cattle and Live stock Regulations 1998"@en-AU ;
    dct:isPartOf F1998B00137:28 ;
    dct:isReferencedBy F1998B00137: ;
    rdfs:comment "32  Transitionalobligations about returns under the Primary Industries Levies and Charges Collection Buffalo Cattle and Live stock Regulations 1998 - Abrievated Graph Key: I37"@en-AU ;
    skos:definition "32  Transitionalobligations about returns under the Primary Industries Levies and Charges Collection Buffalo Cattle and Live stock Regulations 1998"@en-AU ;
    skos:narrower F1998B00137:28 ;
    skos:prefLabel "Item I37"@en-AU ;
    dcat:accessURL <https://www.legislation.gov.au/F1998B00137/2024-07-06/2024-07-06/text/original/epub/OEBPS/document_1/document_1.html#_Toc171769270> ;
    dcat:landingPage "https://www.legislation.gov.au/F1998B00137/2024-07-06/2024-07-06/text/original/epub/OEBPS/document_1/document_1.html#_Toc171769270"^^xsd:anyURI ;
    dcat:theme legcons:Item .

F1998B00137:39 a legcons:Item,
        owl:Class,
        dcat:Resource ;
    rdfs:label "Item - I39 33  Meaning of expressions for Part"@en-AU ;
    dct:isPartOf F1998B00137:38 ;
    dct:isReferencedBy F1998B00137: ;
    rdfs:comment "33  Meaning of expressions for Part - Abrievated Graph Key: I39"@en-AU ;
    skos:definition "33  Meaning of expressions for Part"@en-AU ;
    skos:narrower F1998B00137:38 ;
    skos:prefLabel "Item I39"@en-AU ;
    dcat:accessURL <https://www.legislation.gov.au/F1998B00137/2024-07-06/2024-07-06/text/original/epub/OEBPS/document_1/document_1.html#_Toc171769272> ;
    dcat:landingPage "https://www.legislation.gov.au/F1998B00137/2024-07-06/2024-07-06/text/original/epub/OEBPS/document_1/document_1.html#_Toc171769272"^^xsd:anyURI ;
    dcat:theme legcons:Item .

F1998B00137:4 a legcons:Item,
        owl:Class,
        dcat:Resource ;
    rdfs:label "Item - I4 3 A  Net GST not included in price of product"@en-AU ;
    dct:isPartOf F1998B00137:1 ;
    dct:isReferencedBy F1998B00137: ;
    rdfs:comment "3 A  Net GST not included in price of product - Abrievated Graph Key: I4"@en-AU ;
    skos:definition "3 A  Net GST not included in price of product"@en-AU ;
    skos:narrower F1998B00137:1 ;
    skos:prefLabel "Item I4"@en-AU ;
    dcat:accessURL <https://www.legislation.gov.au/F1998B00137/2024-07-06/2024-07-06/text/original/epub/OEBPS/document_1/document_1.html#_Toc171769237> ;
    dcat:landingPage "https://www.legislation.gov.au/F1998B00137/2024-07-06/2024-07-06/text/original/epub/OEBPS/document_1/document_1.html#_Toc171769237"^^xsd:anyURI ;
    dcat:theme legcons:Item .

F1998B00137:40 a legcons:Item,
        owl:Class,
        dcat:Resource ;
    rdfs:label "Item - I40 33 A  Meaning of eligible coarse grain"@en-AU ;
    dct:isPartOf F1998B00137:38 ;
    dct:isReferencedBy F1998B00137: ;
    rdfs:comment "33 A  Meaning of eligible coarse grain - Abrievated Graph Key: I40"@en-AU ;
    skos:definition "33 A  Meaning of eligible coarse grain"@en-AU ;
    skos:narrower F1998B00137:38 ;
    skos:prefLabel "Item I40"@en-AU ;
    dcat:accessURL <https://www.legislation.gov.au/F1998B00137/2024-07-06/2024-07-06/text/original/epub/OEBPS/document_1/document_1.html#_Toc171769273> ;
    dcat:landingPage "https://www.legislation.gov.au/F1998B00137/2024-07-06/2024-07-06/text/original/epub/OEBPS/document_1/document_1.html#_Toc171769273"^^xsd:anyURI ;
    dcat:theme legcons:Item .

F1998B00137:41 a legcons:Item,
        owl:Class,
        dcat:Resource ;
    rdfs:label "Item - I41 34  Meaning of value"@en-AU ;
    dct:isPartOf F1998B00137:38 ;
    dct:isReferencedBy F1998B00137: ;
    rdfs:comment "34  Meaning of value - Abrievated Graph Key: I41"@en-AU ;
    skos:definition "34  Meaning of value"@en-AU ;
    skos:narrower F1998B00137:38 ;
    skos:prefLabel "Item I41"@en-AU ;
    dcat:accessURL <https://www.legislation.gov.au/F1998B00137/2024-07-06/2024-07-06/text/original/epub/OEBPS/document_1/document_1.html#_Toc171769274> ;
    dcat:landingPage "https://www.legislation.gov.au/F1998B00137/2024-07-06/2024-07-06/text/original/epub/OEBPS/document_1/document_1.html#_Toc171769274"^^xsd:anyURI ;
    dcat:theme legcons:Item .

F1998B00137:42 a legcons:Item,
        owl:Class,
        dcat:Resource ;
    rdfs:label "Item - I42 35  Incorporation with Schedule 8 to the Collection Regulations"@en-AU ;
    dct:isPartOf F1998B00137:38 ;
    dct:isReferencedBy F1998B00137: ;
    rdfs:comment "35  Incorporation with Schedule 8 to the Collection Regulations - Abrievated Graph Key: I42"@en-AU ;
    skos:definition "35  Incorporation with Schedule 8 to the Collection Regulations"@en-AU ;
    skos:narrower F1998B00137:38 ;
    skos:prefLabel "Item I42"@en-AU ;
    dcat:accessURL <https://www.legislation.gov.au/F1998B00137/2024-07-06/2024-07-06/text/original/epub/OEBPS/document_1/document_1.html#_Toc171769275> ;
    dcat:landingPage "https://www.legislation.gov.au/F1998B00137/2024-07-06/2024-07-06/text/original/epub/OEBPS/document_1/document_1.html#_Toc171769275"^^xsd:anyURI ;
    dcat:theme legcons:Item .

F1998B00137:43 a legcons:Item,
        owl:Class,
        dcat:Resource ;
    rdfs:label "Item - I43 36  Rate of NRS excise levy for eligible coarse grain"@en-AU ;
    dct:isPartOf F1998B00137:38 ;
    dct:isReferencedBy F1998B00137: ;
    rdfs:comment "36  Rate of NRS excise levy for eligible coarse grain - Abrievated Graph Key: I43"@en-AU ;
    skos:definition "36  Rate of NRS excise levy for eligible coarse grain"@en-AU ;
    skos:narrower F1998B00137:38 ;
    skos:prefLabel "Item I43"@en-AU ;
    dcat:accessURL <https://www.legislation.gov.au/F1998B00137/2024-07-06/2024-07-06/text/original/epub/OEBPS/document_1/document_1.html#_Toc171769276> ;
    dcat:landingPage "https://www.legislation.gov.au/F1998B00137/2024-07-06/2024-07-06/text/original/epub/OEBPS/document_1/document_1.html#_Toc171769276"^^xsd:anyURI ;
    dcat:theme legcons:Item .

F1998B00137:44 a legcons:Item,
        owl:Class,
        dcat:Resource ;
    rdfs:label "Item - I44 37  When levy is due for payment Collection Act s 6"@en-AU ;
    dct:isPartOf F1998B00137:38 ;
    dct:isReferencedBy F1998B00137: ;
    rdfs:comment "37  When levy is due for payment Collection Act s 6 - Abrievated Graph Key: I44"@en-AU ;
    skos:definition "37  When levy is due for payment Collection Act s 6"@en-AU ;
    skos:narrower F1998B00137:38 ;
    skos:prefLabel "Item I44"@en-AU ;
    dcat:accessURL <https://www.legislation.gov.au/F1998B00137/2024-07-06/2024-07-06/text/original/epub/OEBPS/document_1/document_1.html#_Toc171769277> ;
    dcat:landingPage "https://www.legislation.gov.au/F1998B00137/2024-07-06/2024-07-06/text/original/epub/OEBPS/document_1/document_1.html#_Toc171769277"^^xsd:anyURI ;
    dcat:theme legcons:Item .

F1998B00137:45 a legcons:Item,
        owl:Class,
        dcat:Resource ;
    rdfs:label "Item - I45 38  Information in returns under Schedule 8 to the Collection Regulations"@en-AU ;
    dct:isPartOf F1998B00137:38 ;
    dct:isReferencedBy F1998B00137: ;
    rdfs:comment "38  Information in returns under Schedule 8 to the Collection Regulations - Abrievated Graph Key: I45"@en-AU ;
    skos:definition "38  Information in returns under Schedule 8 to the Collection Regulations"@en-AU ;
    skos:narrower F1998B00137:38 ;
    skos:prefLabel "Item I45"@en-AU ;
    dcat:accessURL <https://www.legislation.gov.au/F1998B00137/2024-07-06/2024-07-06/text/original/epub/OEBPS/document_1/document_1.html#_Toc171769278> ;
    dcat:landingPage "https://www.legislation.gov.au/F1998B00137/2024-07-06/2024-07-06/text/original/epub/OEBPS/document_1/document_1.html#_Toc171769278"^^xsd:anyURI ;
    dcat:theme legcons:Item .

F1998B00137:46 a legcons:Item,
        owl:Class,
        dcat:Resource ;
    rdfs:label "Item - I46 39  Information in records under Schedule 8 to the Collection Regulations"@en-AU ;
    dct:isPartOf F1998B00137:38 ;
    dct:isReferencedBy F1998B00137: ;
    rdfs:comment "39  Information in records under Schedule 8 to the Collection Regulations - Abrievated Graph Key: I46"@en-AU ;
    skos:definition "39  Information in records under Schedule 8 to the Collection Regulations"@en-AU ;
    skos:narrower F1998B00137:38 ;
    skos:prefLabel "Item I46"@en-AU ;
    dcat:accessURL <https://www.legislation.gov.au/F1998B00137/2024-07-06/2024-07-06/text/original/epub/OEBPS/document_1/document_1.html#_Toc171769279> ;
    dcat:landingPage "https://www.legislation.gov.au/F1998B00137/2024-07-06/2024-07-06/text/original/epub/OEBPS/document_1/document_1.html#_Toc171769279"^^xsd:anyURI ;
    dcat:theme legcons:Item .

F1998B00137:48 a legcons:Item,
        owl:Class,
        dcat:Resource ;
    rdfs:label "Item - I48 40  Meaning of expressions for Part"@en-AU ;
    dct:isPartOf F1998B00137:47 ;
    dct:isReferencedBy F1998B00137: ;
    rdfs:comment "40  Meaning of expressions for Part - Abrievated Graph Key: I48"@en-AU ;
    skos:definition "40  Meaning of expressions for Part"@en-AU ;
    skos:narrower F1998B00137:47 ;
    skos:prefLabel "Item I48"@en-AU ;
    dcat:accessURL <https://www.legislation.gov.au/F1998B00137/2024-07-06/2024-07-06/text/original/epub/OEBPS/document_1/document_1.html#_Toc171769281> ;
    dcat:landingPage "https://www.legislation.gov.au/F1998B00137/2024-07-06/2024-07-06/text/original/epub/OEBPS/document_1/document_1.html#_Toc171769281"^^xsd:anyURI ;
    dcat:theme legcons:Item .

F1998B00137:49 a legcons:Item,
        owl:Class,
        dcat:Resource ;
    rdfs:label "Item - I49 41  Incorporation with Schedule 10 to the Collection Regulations"@en-AU ;
    dct:isPartOf F1998B00137:47 ;
    dct:isReferencedBy F1998B00137: ;
    rdfs:comment "41  Incorporation with Schedule 10 to the Collection Regulations - Abrievated Graph Key: I49"@en-AU ;
    skos:definition "41  Incorporation with Schedule 10 to the Collection Regulations"@en-AU ;
    skos:narrower F1998B00137:47 ;
    skos:prefLabel "Item I49"@en-AU ;
    dcat:accessURL <https://www.legislation.gov.au/F1998B00137/2024-07-06/2024-07-06/text/original/epub/OEBPS/document_1/document_1.html#_Toc171769282> ;
    dcat:landingPage "https://www.legislation.gov.au/F1998B00137/2024-07-06/2024-07-06/text/original/epub/OEBPS/document_1/document_1.html#_Toc171769282"^^xsd:anyURI ;
    dcat:theme legcons:Item .

F1998B00137:5 a legcons:Item,
        owl:Class,
        dcat:Resource ;
    rdfs:label "Item - I5 4  Incorporation with the Collection Regulations"@en-AU ;
    dct:isPartOf F1998B00137:1 ;
    dct:isReferencedBy F1998B00137: ;
    rdfs:comment "4  Incorporation with the Collection Regulations - Abrievated Graph Key: I5"@en-AU ;
    skos:definition "4  Incorporation with the Collection Regulations"@en-AU ;
    skos:narrower F1998B00137:1 ;
    skos:prefLabel "Item I5"@en-AU ;
    dcat:accessURL <https://www.legislation.gov.au/F1998B00137/2024-07-06/2024-07-06/text/original/epub/OEBPS/document_1/document_1.html#_Toc171769238> ;
    dcat:landingPage "https://www.legislation.gov.au/F1998B00137/2024-07-06/2024-07-06/text/original/epub/OEBPS/document_1/document_1.html#_Toc171769238"^^xsd:anyURI ;
    dcat:theme legcons:Item .

F1998B00137:50 a legcons:Item,
        owl:Class,
        dcat:Resource ;
    rdfs:label "Item - I50 43  When levy is due for payment Collection Act s 6"@en-AU ;
    dct:isPartOf F1998B00137:47 ;
    dct:isReferencedBy F1998B00137: ;
    rdfs:comment "43  When levy is due for payment Collection Act s 6 - Abrievated Graph Key: I50"@en-AU ;
    skos:definition "43  When levy is due for payment Collection Act s 6"@en-AU ;
    skos:narrower F1998B00137:47 ;
    skos:prefLabel "Item I50"@en-AU ;
    dcat:accessURL <https://www.legislation.gov.au/F1998B00137/2024-07-06/2024-07-06/text/original/epub/OEBPS/document_1/document_1.html#_Toc171769283> ;
    dcat:landingPage "https://www.legislation.gov.au/F1998B00137/2024-07-06/2024-07-06/text/original/epub/OEBPS/document_1/document_1.html#_Toc171769283"^^xsd:anyURI ;
    dcat:theme legcons:Item .

F1998B00137:51 a legcons:Item,
        owl:Class,
        dcat:Resource ;
    rdfs:label "Item - I51 44  Information in returns under Schedule 10 to the Collection Regulations"@en-AU ;
    dct:isPartOf F1998B00137:47 ;
    dct:isReferencedBy F1998B00137: ;
    rdfs:comment "44  Information in returns under Schedule 10 to the Collection Regulations - Abrievated Graph Key: I51"@en-AU ;
    skos:definition "44  Information in returns under Schedule 10 to the Collection Regulations"@en-AU ;
    skos:narrower F1998B00137:47 ;
    skos:prefLabel "Item I51"@en-AU ;
    dcat:accessURL <https://www.legislation.gov.au/F1998B00137/2024-07-06/2024-07-06/text/original/epub/OEBPS/document_1/document_1.html#_Toc171769284> ;
    dcat:landingPage "https://www.legislation.gov.au/F1998B00137/2024-07-06/2024-07-06/text/original/epub/OEBPS/document_1/document_1.html#_Toc171769284"^^xsd:anyURI ;
    dcat:theme legcons:Item .

F1998B00137:52 a legcons:Item,
        owl:Class,
        dcat:Resource ;
    rdfs:label "Item - I52 45  Information in records under Schedule 10 to the Collection Regulations"@en-AU ;
    dct:isPartOf F1998B00137:47 ;
    dct:isReferencedBy F1998B00137: ;
    rdfs:comment "45  Information in records under Schedule 10 to the Collection Regulations - Abrievated Graph Key: I52"@en-AU ;
    skos:definition "45  Information in records under Schedule 10 to the Collection Regulations"@en-AU ;
    skos:narrower F1998B00137:47 ;
    skos:prefLabel "Item I52"@en-AU ;
    dcat:accessURL <https://www.legislation.gov.au/F1998B00137/2024-07-06/2024-07-06/text/original/epub/OEBPS/document_1/document_1.html#_Toc171769285> ;
    dcat:landingPage "https://www.legislation.gov.au/F1998B00137/2024-07-06/2024-07-06/text/original/epub/OEBPS/document_1/document_1.html#_Toc171769285"^^xsd:anyURI ;
    dcat:theme legcons:Item .

F1998B00137:54 a legcons:Item,
        owl:Class,
        dcat:Resource ;
    rdfs:label "Item - I54 46  Meaning of expressions for Part"@en-AU ;
    dct:isPartOf F1998B00137:53 ;
    dct:isReferencedBy F1998B00137: ;
    rdfs:comment "46  Meaning of expressions for Part - Abrievated Graph Key: I54"@en-AU ;
    skos:definition "46  Meaning of expressions for Part"@en-AU ;
    skos:narrower F1998B00137:53 ;
    skos:prefLabel "Item I54"@en-AU ;
    dcat:accessURL <https://www.legislation.gov.au/F1998B00137/2024-07-06/2024-07-06/text/original/epub/OEBPS/document_1/document_1.html#_Toc171769287> ;
    dcat:landingPage "https://www.legislation.gov.au/F1998B00137/2024-07-06/2024-07-06/text/original/epub/OEBPS/document_1/document_1.html#_Toc171769287"^^xsd:anyURI ;
    dcat:theme legcons:Item .

F1998B00137:55 a legcons:Item,
        owl:Class,
        dcat:Resource ;
    rdfs:label "Item - I55 47  Incorporation with Schedule 14 and Part 9 of Schedule 22 to the Collection Regulations"@en-AU ;
    dct:isPartOf F1998B00137:53 ;
    dct:isReferencedBy F1998B00137: ;
    rdfs:comment "47  Incorporation with Schedule 14 and Part 9 of Schedule 22 to the Collection Regulations - Abrievated Graph Key: I55"@en-AU ;
    skos:definition "47  Incorporation with Schedule 14 and Part 9 of Schedule 22 to the Collection Regulations"@en-AU ;
    skos:narrower F1998B00137:53 ;
    skos:prefLabel "Item I55"@en-AU ;
    dcat:accessURL <https://www.legislation.gov.au/F1998B00137/2024-07-06/2024-07-06/text/original/epub/OEBPS/document_1/document_1.html#_Toc171769288> ;
    dcat:landingPage "https://www.legislation.gov.au/F1998B00137/2024-07-06/2024-07-06/text/original/epub/OEBPS/document_1/document_1.html#_Toc171769288"^^xsd:anyURI ;
    dcat:theme legcons:Item .

F1998B00137:56 a legcons:Item,
        owl:Class,
        dcat:Resource ;
    rdfs:label "Item - I56 53  When levy is due for payment Collection Act s 6"@en-AU ;
    dct:isPartOf F1998B00137:53 ;
    dct:isReferencedBy F1998B00137: ;
    rdfs:comment "53  When levy is due for payment Collection Act s 6 - Abrievated Graph Key: I56"@en-AU ;
    skos:definition "53  When levy is due for payment Collection Act s 6"@en-AU ;
    skos:narrower F1998B00137:53 ;
    skos:prefLabel "Item I56"@en-AU ;
    dcat:accessURL <https://www.legislation.gov.au/F1998B00137/2024-07-06/2024-07-06/text/original/epub/OEBPS/document_1/document_1.html#_Toc171769289> ;
    dcat:landingPage "https://www.legislation.gov.au/F1998B00137/2024-07-06/2024-07-06/text/original/epub/OEBPS/document_1/document_1.html#_Toc171769289"^^xsd:anyURI ;
    dcat:theme legcons:Item .

F1998B00137:57 a legcons:Item,
        owl:Class,
        dcat:Resource ;
    rdfs:label "Item - I57 54  Information in returns under Schedule 14 to the Collection Regulations"@en-AU ;
    dct:isPartOf F1998B00137:53 ;
    dct:isReferencedBy F1998B00137: ;
    rdfs:comment "54  Information in returns under Schedule 14 to the Collection Regulations - Abrievated Graph Key: I57"@en-AU ;
    skos:definition "54  Information in returns under Schedule 14 to the Collection Regulations"@en-AU ;
    skos:narrower F1998B00137:53 ;
    skos:prefLabel "Item I57"@en-AU ;
    dcat:accessURL <https://www.legislation.gov.au/F1998B00137/2024-07-06/2024-07-06/text/original/epub/OEBPS/document_1/document_1.html#_Toc171769290> ;
    dcat:landingPage "https://www.legislation.gov.au/F1998B00137/2024-07-06/2024-07-06/text/original/epub/OEBPS/document_1/document_1.html#_Toc171769290"^^xsd:anyURI ;
    dcat:theme legcons:Item .

F1998B00137:58 a legcons:Item,
        owl:Class,
        dcat:Resource ;
    rdfs:label "Item - I58 55  Information in returns under Part 9 of Schedule 22 to the Collection Regulations"@en-AU ;
    dct:isPartOf F1998B00137:53 ;
    dct:isReferencedBy F1998B00137: ;
    rdfs:comment "55  Information in returns under Part 9 of Schedule 22 to the Collection Regulations - Abrievated Graph Key: I58"@en-AU ;
    skos:definition "55  Information in returns under Part 9 of Schedule 22 to the Collection Regulations"@en-AU ;
    skos:narrower F1998B00137:53 ;
    skos:prefLabel "Item I58"@en-AU ;
    dcat:accessURL <https://www.legislation.gov.au/F1998B00137/2024-07-06/2024-07-06/text/original/epub/OEBPS/document_1/document_1.html#_Toc171769291> ;
    dcat:landingPage "https://www.legislation.gov.au/F1998B00137/2024-07-06/2024-07-06/text/original/epub/OEBPS/document_1/document_1.html#_Toc171769291"^^xsd:anyURI ;
    dcat:theme legcons:Item .

F1998B00137:59 a legcons:Item,
        owl:Class,
        dcat:Resource ;
    rdfs:label "Item - I59 56  Information in records under Schedule 14 to the Collection Regulations"@en-AU ;
    dct:isPartOf F1998B00137:53 ;
    dct:isReferencedBy F1998B00137: ;
    rdfs:comment "56  Information in records under Schedule 14 to the Collection Regulations - Abrievated Graph Key: I59"@en-AU ;
    skos:definition "56  Information in records under Schedule 14 to the Collection Regulations"@en-AU ;
    skos:narrower F1998B00137:53 ;
    skos:prefLabel "Item I59"@en-AU ;
    dcat:accessURL <https://www.legislation.gov.au/F1998B00137/2024-07-06/2024-07-06/text/original/epub/OEBPS/document_1/document_1.html#_Toc171769292> ;
    dcat:landingPage "https://www.legislation.gov.au/F1998B00137/2024-07-06/2024-07-06/text/original/epub/OEBPS/document_1/document_1.html#_Toc171769292"^^xsd:anyURI ;
    dcat:theme legcons:Item .

F1998B00137:60 a legcons:Item,
        owl:Class,
        dcat:Resource ;
    rdfs:label "Item - I60 57  Information in records under Part 9 of Schedule 22 to the Collection Regulations"@en-AU ;
    dct:isPartOf F1998B00137:53 ;
    dct:isReferencedBy F1998B00137: ;
    rdfs:comment "57  Information in records under Part 9 of Schedule 22 to the Collection Regulations - Abrievated Graph Key: I60"@en-AU ;
    skos:definition "57  Information in records under Part 9 of Schedule 22 to the Collection Regulations"@en-AU ;
    skos:narrower F1998B00137:53 ;
    skos:prefLabel "Item I60"@en-AU ;
    dcat:accessURL <https://www.legislation.gov.au/F1998B00137/2024-07-06/2024-07-06/text/original/epub/OEBPS/document_1/document_1.html#_Toc171769293> ;
    dcat:landingPage "https://www.legislation.gov.au/F1998B00137/2024-07-06/2024-07-06/text/original/epub/OEBPS/document_1/document_1.html#_Toc171769293"^^xsd:anyURI ;
    dcat:theme legcons:Item .

F1998B00137:62 a legcons:Item,
        owl:Class,
        dcat:Resource ;
    rdfs:label "Item - I62 58  Meaning of expressions for Part"@en-AU ;
    dct:isPartOf F1998B00137:61 ;
    dct:isReferencedBy F1998B00137: ;
    rdfs:comment "58  Meaning of expressions for Part - Abrievated Graph Key: I62"@en-AU ;
    skos:definition "58  Meaning of expressions for Part"@en-AU ;
    skos:narrower F1998B00137:61 ;
    skos:prefLabel "Item I62"@en-AU ;
    dcat:accessURL <https://www.legislation.gov.au/F1998B00137/2024-07-06/2024-07-06/text/original/epub/OEBPS/document_1/document_1.html#_Toc171769295> ;
    dcat:landingPage "https://www.legislation.gov.au/F1998B00137/2024-07-06/2024-07-06/text/original/epub/OEBPS/document_1/document_1.html#_Toc171769295"^^xsd:anyURI ;
    dcat:theme legcons:Item .

F1998B00137:63 a legcons:Item,
        owl:Class,
        dcat:Resource ;
    rdfs:label "Item - I63 59  Levy year Collection Act s 41 definition of levy year"@en-AU ;
    dct:isPartOf F1998B00137:61 ;
    dct:isReferencedBy F1998B00137: ;
    rdfs:comment "59  Levy year Collection Act s 41 definition of levy year - Abrievated Graph Key: I63"@en-AU ;
    skos:definition "59  Levy year Collection Act s 41 definition of levy year"@en-AU ;
    skos:narrower F1998B00137:61 ;
    skos:prefLabel "Item I63"@en-AU ;
    dcat:accessURL <https://www.legislation.gov.au/F1998B00137/2024-07-06/2024-07-06/text/original/epub/OEBPS/document_1/document_1.html#_Toc171769296> ;
    dcat:landingPage "https://www.legislation.gov.au/F1998B00137/2024-07-06/2024-07-06/text/original/epub/OEBPS/document_1/document_1.html#_Toc171769296"^^xsd:anyURI ;
    dcat:theme legcons:Item .

F1998B00137:64 a legcons:Item,
        owl:Class,
        dcat:Resource ;
    rdfs:label "Item - I64 60  Processor is producer for Collection Act"@en-AU ;
    dct:isPartOf F1998B00137:61 ;
    dct:isReferencedBy F1998B00137: ;
    rdfs:comment "60  Processor is producer for Collection Act - Abrievated Graph Key: I64"@en-AU ;
    skos:definition "60  Processor is producer for Collection Act"@en-AU ;
    skos:narrower F1998B00137:61 ;
    skos:prefLabel "Item I64"@en-AU ;
    dcat:accessURL <https://www.legislation.gov.au/F1998B00137/2024-07-06/2024-07-06/text/original/epub/OEBPS/document_1/document_1.html#_Toc171769297> ;
    dcat:landingPage "https://www.legislation.gov.au/F1998B00137/2024-07-06/2024-07-06/text/original/epub/OEBPS/document_1/document_1.html#_Toc171769297"^^xsd:anyURI ;
    dcat:theme legcons:Item .

F1998B00137:65 a legcons:Item,
        owl:Class,
        dcat:Resource ;
    rdfs:label "Item - I65 61  Rate of NRS excise levy on game animals"@en-AU ;
    dct:isPartOf F1998B00137:61 ;
    dct:isReferencedBy F1998B00137: ;
    rdfs:comment "61  Rate of NRS excise levy on game animals - Abrievated Graph Key: I65"@en-AU ;
    skos:definition "61  Rate of NRS excise levy on game animals"@en-AU ;
    skos:narrower F1998B00137:61 ;
    skos:prefLabel "Item I65"@en-AU ;
    dcat:accessURL <https://www.legislation.gov.au/F1998B00137/2024-07-06/2024-07-06/text/original/epub/OEBPS/document_1/document_1.html#_Toc171769298> ;
    dcat:landingPage "https://www.legislation.gov.au/F1998B00137/2024-07-06/2024-07-06/text/original/epub/OEBPS/document_1/document_1.html#_Toc171769298"^^xsd:anyURI ;
    dcat:theme legcons:Item .

F1998B00137:66 a legcons:Item,
        owl:Class,
        dcat:Resource ;
    rdfs:label "Item - I66 62  When levy is due for payment Collection Act s 6"@en-AU ;
    dct:isPartOf F1998B00137:61 ;
    dct:isReferencedBy F1998B00137: ;
    rdfs:comment "62  When levy is due for payment Collection Act s 6 - Abrievated Graph Key: I66"@en-AU ;
    skos:definition "62  When levy is due for payment Collection Act s 6"@en-AU ;
    skos:narrower F1998B00137:61 ;
    skos:prefLabel "Item I66"@en-AU ;
    dcat:accessURL <https://www.legislation.gov.au/F1998B00137/2024-07-06/2024-07-06/text/original/epub/OEBPS/document_1/document_1.html#_Toc171769299> ;
    dcat:landingPage "https://www.legislation.gov.au/F1998B00137/2024-07-06/2024-07-06/text/original/epub/OEBPS/document_1/document_1.html#_Toc171769299"^^xsd:anyURI ;
    dcat:theme legcons:Item .

F1998B00137:67 a legcons:Item,
        owl:Class,
        dcat:Resource ;
    rdfs:label "Item - I67 63  Who must give Secretary return"@en-AU ;
    dct:isPartOf F1998B00137:61 ;
    dct:isReferencedBy F1998B00137: ;
    rdfs:comment "63  Who must give Secretary return - Abrievated Graph Key: I67"@en-AU ;
    skos:definition "63  Who must give Secretary return"@en-AU ;
    skos:narrower F1998B00137:61 ;
    skos:prefLabel "Item I67"@en-AU ;
    dcat:accessURL <https://www.legislation.gov.au/F1998B00137/2024-07-06/2024-07-06/text/original/epub/OEBPS/document_1/document_1.html#_Toc171769300> ;
    dcat:landingPage "https://www.legislation.gov.au/F1998B00137/2024-07-06/2024-07-06/text/original/epub/OEBPS/document_1/document_1.html#_Toc171769300"^^xsd:anyURI ;
    dcat:theme legcons:Item .

F1998B00137:68 a legcons:Item,
        owl:Class,
        dcat:Resource ;
    rdfs:label "Item - I68 64  What must be in return"@en-AU ;
    dct:isPartOf F1998B00137:61 ;
    dct:isReferencedBy F1998B00137: ;
    rdfs:comment "64  What must be in return - Abrievated Graph Key: I68"@en-AU ;
    skos:definition "64  What must be in return"@en-AU ;
    skos:narrower F1998B00137:61 ;
    skos:prefLabel "Item I68"@en-AU ;
    dcat:accessURL <https://www.legislation.gov.au/F1998B00137/2024-07-06/2024-07-06/text/original/epub/OEBPS/document_1/document_1.html#_Toc171769301> ;
    dcat:landingPage "https://www.legislation.gov.au/F1998B00137/2024-07-06/2024-07-06/text/original/epub/OEBPS/document_1/document_1.html#_Toc171769301"^^xsd:anyURI ;
    dcat:theme legcons:Item .

F1998B00137:69 a legcons:Item,
        owl:Class,
        dcat:Resource ;
    rdfs:label "Item - I69 65  When and how return must be given to Secretary"@en-AU ;
    dct:isPartOf F1998B00137:61 ;
    dct:isReferencedBy F1998B00137: ;
    rdfs:comment "65  When and how return must be given to Secretary - Abrievated Graph Key: I69"@en-AU ;
    skos:definition "65  When and how return must be given to Secretary"@en-AU ;
    skos:narrower F1998B00137:61 ;
    skos:prefLabel "Item I69"@en-AU ;
    dcat:accessURL <https://www.legislation.gov.au/F1998B00137/2024-07-06/2024-07-06/text/original/epub/OEBPS/document_1/document_1.html#_Toc171769302> ;
    dcat:landingPage "https://www.legislation.gov.au/F1998B00137/2024-07-06/2024-07-06/text/original/epub/OEBPS/document_1/document_1.html#_Toc171769302"^^xsd:anyURI ;
    dcat:theme legcons:Item .

F1998B00137:7 a legcons:Item,
        owl:Class,
        dcat:Resource ;
    rdfs:label "Item - I7 5  Meaning of expressions for Part"@en-AU ;
    dct:isPartOf F1998B00137:6 ;
    dct:isReferencedBy F1998B00137: ;
    rdfs:comment "5  Meaning of expressions for Part - Abrievated Graph Key: I7"@en-AU ;
    skos:definition "5  Meaning of expressions for Part"@en-AU ;
    skos:narrower F1998B00137:6 ;
    skos:prefLabel "Item I7"@en-AU ;
    dcat:accessURL <https://www.legislation.gov.au/F1998B00137/2024-07-06/2024-07-06/text/original/epub/OEBPS/document_1/document_1.html#_Toc171769240> ;
    dcat:landingPage "https://www.legislation.gov.au/F1998B00137/2024-07-06/2024-07-06/text/original/epub/OEBPS/document_1/document_1.html#_Toc171769240"^^xsd:anyURI ;
    dcat:theme legcons:Item .

F1998B00137:70 a legcons:Item,
        owl:Class,
        dcat:Resource ;
    rdfs:label "Item - I70 66  What records must be kept"@en-AU ;
    dct:isPartOf F1998B00137:61 ;
    dct:isReferencedBy F1998B00137: ;
    rdfs:comment "66  What records must be kept - Abrievated Graph Key: I70"@en-AU ;
    skos:definition "66  What records must be kept"@en-AU ;
    skos:narrower F1998B00137:61 ;
    skos:prefLabel "Item I70"@en-AU ;
    dcat:accessURL <https://www.legislation.gov.au/F1998B00137/2024-07-06/2024-07-06/text/original/epub/OEBPS/document_1/document_1.html#_Toc171769303> ;
    dcat:landingPage "https://www.legislation.gov.au/F1998B00137/2024-07-06/2024-07-06/text/original/epub/OEBPS/document_1/document_1.html#_Toc171769303"^^xsd:anyURI ;
    dcat:theme legcons:Item .

F1998B00137:71 a legcons:Item,
        owl:Class,
        dcat:Resource ;
    rdfs:label "Item - I71 67  How long records must be retained"@en-AU ;
    dct:isPartOf F1998B00137:61 ;
    dct:isReferencedBy F1998B00137: ;
    rdfs:comment "67  How long records must be retained - Abrievated Graph Key: I71"@en-AU ;
    skos:definition "67  How long records must be retained"@en-AU ;
    skos:narrower F1998B00137:61 ;
    skos:prefLabel "Item I71"@en-AU ;
    dcat:accessURL <https://www.legislation.gov.au/F1998B00137/2024-07-06/2024-07-06/text/original/epub/OEBPS/document_1/document_1.html#_Toc171769304> ;
    dcat:landingPage "https://www.legislation.gov.au/F1998B00137/2024-07-06/2024-07-06/text/original/epub/OEBPS/document_1/document_1.html#_Toc171769304"^^xsd:anyURI ;
    dcat:theme legcons:Item .

F1998B00137:72 a legcons:Item,
        owl:Class,
        dcat:Resource ;
    rdfs:label "Item - I72 68  Transitionalobligations about returns under former regulations"@en-AU ;
    dct:isPartOf F1998B00137:61 ;
    dct:isReferencedBy F1998B00137: ;
    rdfs:comment "68  Transitionalobligations about returns under former regulations - Abrievated Graph Key: I72"@en-AU ;
    skos:definition "68  Transitionalobligations about returns under former regulations"@en-AU ;
    skos:narrower F1998B00137:61 ;
    skos:prefLabel "Item I72"@en-AU ;
    dcat:accessURL <https://www.legislation.gov.au/F1998B00137/2024-07-06/2024-07-06/text/original/epub/OEBPS/document_1/document_1.html#_Toc171769305> ;
    dcat:landingPage "https://www.legislation.gov.au/F1998B00137/2024-07-06/2024-07-06/text/original/epub/OEBPS/document_1/document_1.html#_Toc171769305"^^xsd:anyURI ;
    dcat:theme legcons:Item .

F1998B00137:74 a legcons:Item,
        owl:Class,
        dcat:Resource ;
    rdfs:label "Item - I74 69  Meaning of expressions for Part"@en-AU ;
    dct:isPartOf F1998B00137:73 ;
    dct:isReferencedBy F1998B00137: ;
    rdfs:comment "69  Meaning of expressions for Part - Abrievated Graph Key: I74"@en-AU ;
    skos:definition "69  Meaning of expressions for Part"@en-AU ;
    skos:narrower F1998B00137:73 ;
    skos:prefLabel "Item I74"@en-AU ;
    dcat:accessURL <https://www.legislation.gov.au/F1998B00137/2024-07-06/2024-07-06/text/original/epub/OEBPS/document_1/document_1.html#_Toc171769307> ;
    dcat:landingPage "https://www.legislation.gov.au/F1998B00137/2024-07-06/2024-07-06/text/original/epub/OEBPS/document_1/document_1.html#_Toc171769307"^^xsd:anyURI ;
    dcat:theme legcons:Item .

F1998B00137:75 a legcons:Item,
        owl:Class,
        dcat:Resource ;
    rdfs:label "Item - I75 69 A  Meaning of eligible grain legumes"@en-AU ;
    dct:isPartOf F1998B00137:73 ;
    dct:isReferencedBy F1998B00137: ;
    rdfs:comment "69 A  Meaning of eligible grain legumes - Abrievated Graph Key: I75"@en-AU ;
    skos:definition "69 A  Meaning of eligible grain legumes"@en-AU ;
    skos:narrower F1998B00137:73 ;
    skos:prefLabel "Item I75"@en-AU ;
    dcat:accessURL <https://www.legislation.gov.au/F1998B00137/2024-07-06/2024-07-06/text/original/epub/OEBPS/document_1/document_1.html#_Toc171769308> ;
    dcat:landingPage "https://www.legislation.gov.au/F1998B00137/2024-07-06/2024-07-06/text/original/epub/OEBPS/document_1/document_1.html#_Toc171769308"^^xsd:anyURI ;
    dcat:theme legcons:Item .

F1998B00137:76 a legcons:Item,
        owl:Class,
        dcat:Resource ;
    rdfs:label "Item - I76 70  Meaning of value"@en-AU ;
    dct:isPartOf F1998B00137:73 ;
    dct:isReferencedBy F1998B00137: ;
    rdfs:comment "70  Meaning of value - Abrievated Graph Key: I76"@en-AU ;
    skos:definition "70  Meaning of value"@en-AU ;
    skos:narrower F1998B00137:73 ;
    skos:prefLabel "Item I76"@en-AU ;
    dcat:accessURL <https://www.legislation.gov.au/F1998B00137/2024-07-06/2024-07-06/text/original/epub/OEBPS/document_1/document_1.html#_Toc171769309> ;
    dcat:landingPage "https://www.legislation.gov.au/F1998B00137/2024-07-06/2024-07-06/text/original/epub/OEBPS/document_1/document_1.html#_Toc171769309"^^xsd:anyURI ;
    dcat:theme legcons:Item .

F1998B00137:77 a legcons:Item,
        owl:Class,
        dcat:Resource ;
    rdfs:label "Item - I77 71  Incorporation with Schedule 19 to the Collection Regulations"@en-AU ;
    dct:isPartOf F1998B00137:73 ;
    dct:isReferencedBy F1998B00137: ;
    rdfs:comment "71  Incorporation with Schedule 19 to the Collection Regulations - Abrievated Graph Key: I77"@en-AU ;
    skos:definition "71  Incorporation with Schedule 19 to the Collection Regulations"@en-AU ;
    skos:narrower F1998B00137:73 ;
    skos:prefLabel "Item I77"@en-AU ;
    dcat:accessURL <https://www.legislation.gov.au/F1998B00137/2024-07-06/2024-07-06/text/original/epub/OEBPS/document_1/document_1.html#_Toc171769310> ;
    dcat:landingPage "https://www.legislation.gov.au/F1998B00137/2024-07-06/2024-07-06/text/original/epub/OEBPS/document_1/document_1.html#_Toc171769310"^^xsd:anyURI ;
    dcat:theme legcons:Item .

F1998B00137:78 a legcons:Item,
        owl:Class,
        dcat:Resource ;
    rdfs:label "Item - I78 72  Rate of NRS excise levy for eligible grain legumes"@en-AU ;
    dct:isPartOf F1998B00137:73 ;
    dct:isReferencedBy F1998B00137: ;
    rdfs:comment "72  Rate of NRS excise levy for eligible grain legumes - Abrievated Graph Key: I78"@en-AU ;
    skos:definition "72  Rate of NRS excise levy for eligible grain legumes"@en-AU ;
    skos:narrower F1998B00137:73 ;
    skos:prefLabel "Item I78"@en-AU ;
    dcat:accessURL <https://www.legislation.gov.au/F1998B00137/2024-07-06/2024-07-06/text/original/epub/OEBPS/document_1/document_1.html#_Toc171769311> ;
    dcat:landingPage "https://www.legislation.gov.au/F1998B00137/2024-07-06/2024-07-06/text/original/epub/OEBPS/document_1/document_1.html#_Toc171769311"^^xsd:anyURI ;
    dcat:theme legcons:Item .

F1998B00137:79 a legcons:Item,
        owl:Class,
        dcat:Resource ;
    rdfs:label "Item - I79 74  When levy is due for payment Collection Act s 6"@en-AU ;
    dct:isPartOf F1998B00137:73 ;
    dct:isReferencedBy F1998B00137: ;
    rdfs:comment "74  When levy is due for payment Collection Act s 6 - Abrievated Graph Key: I79"@en-AU ;
    skos:definition "74  When levy is due for payment Collection Act s 6"@en-AU ;
    skos:narrower F1998B00137:73 ;
    skos:prefLabel "Item I79"@en-AU ;
    dcat:accessURL <https://www.legislation.gov.au/F1998B00137/2024-07-06/2024-07-06/text/original/epub/OEBPS/document_1/document_1.html#_Toc171769312> ;
    dcat:landingPage "https://www.legislation.gov.au/F1998B00137/2024-07-06/2024-07-06/text/original/epub/OEBPS/document_1/document_1.html#_Toc171769312"^^xsd:anyURI ;
    dcat:theme legcons:Item .

F1998B00137:8 a legcons:Item,
        owl:Class,
        dcat:Resource ;
    rdfs:label "Item - I8 6  Levy year Collection Act s 41 definition of levy year"@en-AU ;
    dct:isPartOf F1998B00137:6 ;
    dct:isReferencedBy F1998B00137: ;
    rdfs:comment "6  Levy year Collection Act s 41 definition of levy year - Abrievated Graph Key: I8"@en-AU ;
    skos:definition "6  Levy year Collection Act s 41 definition of levy year"@en-AU ;
    skos:narrower F1998B00137:6 ;
    skos:prefLabel "Item I8"@en-AU ;
    dcat:accessURL <https://www.legislation.gov.au/F1998B00137/2024-07-06/2024-07-06/text/original/epub/OEBPS/document_1/document_1.html#_Toc171769241> ;
    dcat:landingPage "https://www.legislation.gov.au/F1998B00137/2024-07-06/2024-07-06/text/original/epub/OEBPS/document_1/document_1.html#_Toc171769241"^^xsd:anyURI ;
    dcat:theme legcons:Item .

F1998B00137:80 a legcons:Item,
        owl:Class,
        dcat:Resource ;
    rdfs:label "Item - I80 75  Information in returns under Schedule 19 to the Collection Regulations"@en-AU ;
    dct:isPartOf F1998B00137:73 ;
    dct:isReferencedBy F1998B00137: ;
    rdfs:comment "75  Information in returns under Schedule 19 to the Collection Regulations - Abrievated Graph Key: I80"@en-AU ;
    skos:definition "75  Information in returns under Schedule 19 to the Collection Regulations"@en-AU ;
    skos:narrower F1998B00137:73 ;
    skos:prefLabel "Item I80"@en-AU ;
    dcat:accessURL <https://www.legislation.gov.au/F1998B00137/2024-07-06/2024-07-06/text/original/epub/OEBPS/document_1/document_1.html#_Toc171769313> ;
    dcat:landingPage "https://www.legislation.gov.au/F1998B00137/2024-07-06/2024-07-06/text/original/epub/OEBPS/document_1/document_1.html#_Toc171769313"^^xsd:anyURI ;
    dcat:theme legcons:Item .

F1998B00137:81 a legcons:Item,
        owl:Class,
        dcat:Resource ;
    rdfs:label "Item - I81 76  Information in records under Schedule 19 to the Collection Regulations"@en-AU ;
    dct:isPartOf F1998B00137:73 ;
    dct:isReferencedBy F1998B00137: ;
    rdfs:comment "76  Information in records under Schedule 19 to the Collection Regulations - Abrievated Graph Key: I81"@en-AU ;
    skos:definition "76  Information in records under Schedule 19 to the Collection Regulations"@en-AU ;
    skos:narrower F1998B00137:73 ;
    skos:prefLabel "Item I81"@en-AU ;
    dcat:accessURL <https://www.legislation.gov.au/F1998B00137/2024-07-06/2024-07-06/text/original/epub/OEBPS/document_1/document_1.html#_Toc171769314> ;
    dcat:landingPage "https://www.legislation.gov.au/F1998B00137/2024-07-06/2024-07-06/text/original/epub/OEBPS/document_1/document_1.html#_Toc171769314"^^xsd:anyURI ;
    dcat:theme legcons:Item .

F1998B00137:83 a legcons:Item,
        owl:Class,
        dcat:Resource ;
    rdfs:label "Item - I83 77  Meaning of expressions for Part 9"@en-AU ;
    dct:isPartOf F1998B00137:82 ;
    dct:isReferencedBy F1998B00137: ;
    rdfs:comment "77  Meaning of expressions for Part 9 - Abrievated Graph Key: I83"@en-AU ;
    skos:definition "77  Meaning of expressions for Part 9"@en-AU ;
    skos:narrower F1998B00137:82 ;
    skos:prefLabel "Item I83"@en-AU ;
    dcat:accessURL <https://www.legislation.gov.au/F1998B00137/2024-07-06/2024-07-06/text/original/epub/OEBPS/document_1/document_1.html#_Toc171769316> ;
    dcat:landingPage "https://www.legislation.gov.au/F1998B00137/2024-07-06/2024-07-06/text/original/epub/OEBPS/document_1/document_1.html#_Toc171769316"^^xsd:anyURI ;
    dcat:theme legcons:Item .

F1998B00137:84 a legcons:Item,
        owl:Class,
        dcat:Resource ;
    rdfs:label "Item - I84 78  Incorporation with Schedule 21 to the Collection Regulations"@en-AU ;
    dct:isPartOf F1998B00137:82 ;
    dct:isReferencedBy F1998B00137: ;
    rdfs:comment "78  Incorporation with Schedule 21 to the Collection Regulations - Abrievated Graph Key: I84"@en-AU ;
    skos:definition "78  Incorporation with Schedule 21 to the Collection Regulations"@en-AU ;
    skos:narrower F1998B00137:82 ;
    skos:prefLabel "Item I84"@en-AU ;
    dcat:accessURL <https://www.legislation.gov.au/F1998B00137/2024-07-06/2024-07-06/text/original/epub/OEBPS/document_1/document_1.html#_Toc171769317> ;
    dcat:landingPage "https://www.legislation.gov.au/F1998B00137/2024-07-06/2024-07-06/text/original/epub/OEBPS/document_1/document_1.html#_Toc171769317"^^xsd:anyURI ;
    dcat:theme legcons:Item .

F1998B00137:85 a legcons:Item,
        owl:Class,
        dcat:Resource ;
    rdfs:label "Item - I85 78 A  Exemption from NRS excise levy on honey"@en-AU ;
    dct:isPartOf F1998B00137:82 ;
    dct:isReferencedBy F1998B00137: ;
    rdfs:comment "78 A  Exemption from NRS excise levy on honey - Abrievated Graph Key: I85"@en-AU ;
    skos:definition "78 A  Exemption from NRS excise levy on honey"@en-AU ;
    skos:narrower F1998B00137:82 ;
    skos:prefLabel "Item I85"@en-AU ;
    dcat:accessURL <https://www.legislation.gov.au/F1998B00137/2024-07-06/2024-07-06/text/original/epub/OEBPS/document_1/document_1.html#_Toc171769318> ;
    dcat:landingPage "https://www.legislation.gov.au/F1998B00137/2024-07-06/2024-07-06/text/original/epub/OEBPS/document_1/document_1.html#_Toc171769318"^^xsd:anyURI ;
    dcat:theme legcons:Item .

F1998B00137:86 a legcons:Item,
        owl:Class,
        dcat:Resource ;
    rdfs:label "Item - I86 79  Rate of NRS customs levy on honey"@en-AU ;
    dct:isPartOf F1998B00137:82 ;
    dct:isReferencedBy F1998B00137: ;
    rdfs:comment "79  Rate of NRS customs levy on honey - Abrievated Graph Key: I86"@en-AU ;
    skos:definition "79  Rate of NRS customs levy on honey"@en-AU ;
    skos:narrower F1998B00137:82 ;
    skos:prefLabel "Item I86"@en-AU ;
    dcat:accessURL <https://www.legislation.gov.au/F1998B00137/2024-07-06/2024-07-06/text/original/epub/OEBPS/document_1/document_1.html#_Toc171769319> ;
    dcat:landingPage "https://www.legislation.gov.au/F1998B00137/2024-07-06/2024-07-06/text/original/epub/OEBPS/document_1/document_1.html#_Toc171769319"^^xsd:anyURI ;
    dcat:theme legcons:Item .

F1998B00137:87 a legcons:Item,
        owl:Class,
        dcat:Resource ;
    rdfs:label "Item - I87 80  Rate of NRS excise levy on honey"@en-AU ;
    dct:isPartOf F1998B00137:82 ;
    dct:isReferencedBy F1998B00137: ;
    rdfs:comment "80  Rate of NRS excise levy on honey - Abrievated Graph Key: I87"@en-AU ;
    skos:definition "80  Rate of NRS excise levy on honey"@en-AU ;
    skos:narrower F1998B00137:82 ;
    skos:prefLabel "Item I87"@en-AU ;
    dcat:accessURL <https://www.legislation.gov.au/F1998B00137/2024-07-06/2024-07-06/text/original/epub/OEBPS/document_1/document_1.html#_Toc171769320> ;
    dcat:landingPage "https://www.legislation.gov.au/F1998B00137/2024-07-06/2024-07-06/text/original/epub/OEBPS/document_1/document_1.html#_Toc171769320"^^xsd:anyURI ;
    dcat:theme legcons:Item .

F1998B00137:88 a legcons:Item,
        owl:Class,
        dcat:Resource ;
    rdfs:label "Item - I88 81  When levy is due for payment Collection Act s 6"@en-AU ;
    dct:isPartOf F1998B00137:82 ;
    dct:isReferencedBy F1998B00137: ;
    rdfs:comment "81  When levy is due for payment Collection Act s 6 - Abrievated Graph Key: I88"@en-AU ;
    skos:definition "81  When levy is due for payment Collection Act s 6"@en-AU ;
    skos:narrower F1998B00137:82 ;
    skos:prefLabel "Item I88"@en-AU ;
    dcat:accessURL <https://www.legislation.gov.au/F1998B00137/2024-07-06/2024-07-06/text/original/epub/OEBPS/document_1/document_1.html#_Toc171769321> ;
    dcat:landingPage "https://www.legislation.gov.au/F1998B00137/2024-07-06/2024-07-06/text/original/epub/OEBPS/document_1/document_1.html#_Toc171769321"^^xsd:anyURI ;
    dcat:theme legcons:Item .

F1998B00137:89 a legcons:Item,
        owl:Class,
        dcat:Resource ;
    rdfs:label "Item - I89 82  Information in returns under Schedule 21 to the Collection Regulations"@en-AU ;
    dct:isPartOf F1998B00137:82 ;
    dct:isReferencedBy F1998B00137: ;
    rdfs:comment "82  Information in returns under Schedule 21 to the Collection Regulations - Abrievated Graph Key: I89"@en-AU ;
    skos:definition "82  Information in returns under Schedule 21 to the Collection Regulations"@en-AU ;
    skos:narrower F1998B00137:82 ;
    skos:prefLabel "Item I89"@en-AU ;
    dcat:accessURL <https://www.legislation.gov.au/F1998B00137/2024-07-06/2024-07-06/text/original/epub/OEBPS/document_1/document_1.html#_Toc171769322> ;
    dcat:landingPage "https://www.legislation.gov.au/F1998B00137/2024-07-06/2024-07-06/text/original/epub/OEBPS/document_1/document_1.html#_Toc171769322"^^xsd:anyURI ;
    dcat:theme legcons:Item .

F1998B00137:9 a legcons:Item,
        owl:Class,
        dcat:Resource ;
    rdfs:label "Item - I9 7  Exporter is producer for Collection Act"@en-AU ;
    dct:isPartOf F1998B00137:6 ;
    dct:isReferencedBy F1998B00137: ;
    rdfs:comment "7  Exporter is producer for Collection Act - Abrievated Graph Key: I9"@en-AU ;
    skos:definition "7  Exporter is producer for Collection Act"@en-AU ;
    skos:narrower F1998B00137:6 ;
    skos:prefLabel "Item I9"@en-AU ;
    dcat:accessURL <https://www.legislation.gov.au/F1998B00137/2024-07-06/2024-07-06/text/original/epub/OEBPS/document_1/document_1.html#_Toc171769242> ;
    dcat:landingPage "https://www.legislation.gov.au/F1998B00137/2024-07-06/2024-07-06/text/original/epub/OEBPS/document_1/document_1.html#_Toc171769242"^^xsd:anyURI ;
    dcat:theme legcons:Item .

F1998B00137:90 a legcons:Item,
        owl:Class,
        dcat:Resource ;
    rdfs:label "Item - I90 83  Information in records under Schedule 21 to the Collection Regulations"@en-AU ;
    dct:isPartOf F1998B00137:82 ;
    dct:isReferencedBy F1998B00137: ;
    rdfs:comment "83  Information in records under Schedule 21 to the Collection Regulations - Abrievated Graph Key: I90"@en-AU ;
    skos:definition "83  Information in records under Schedule 21 to the Collection Regulations"@en-AU ;
    skos:narrower F1998B00137:82 ;
    skos:prefLabel "Item I90"@en-AU ;
    dcat:accessURL <https://www.legislation.gov.au/F1998B00137/2024-07-06/2024-07-06/text/original/epub/OEBPS/document_1/document_1.html#_Toc171769323> ;
    dcat:landingPage "https://www.legislation.gov.au/F1998B00137/2024-07-06/2024-07-06/text/original/epub/OEBPS/document_1/document_1.html#_Toc171769323"^^xsd:anyURI ;
    dcat:theme legcons:Item .

F1998B00137:92 a legcons:Item,
        owl:Class,
        dcat:Resource ;
    rdfs:label "Item - I92 84  Meaning of expressions for Part"@en-AU ;
    dct:isPartOf F1998B00137:91 ;
    dct:isReferencedBy F1998B00137: ;
    rdfs:comment "84  Meaning of expressions for Part - Abrievated Graph Key: I92"@en-AU ;
    skos:definition "84  Meaning of expressions for Part"@en-AU ;
    skos:narrower F1998B00137:91 ;
    skos:prefLabel "Item I92"@en-AU ;
    dcat:accessURL <https://www.legislation.gov.au/F1998B00137/2024-07-06/2024-07-06/text/original/epub/OEBPS/document_1/document_1.html#_Toc171769325> ;
    dcat:landingPage "https://www.legislation.gov.au/F1998B00137/2024-07-06/2024-07-06/text/original/epub/OEBPS/document_1/document_1.html#_Toc171769325"^^xsd:anyURI ;
    dcat:theme legcons:Item .

F1998B00137:93 a legcons:Item,
        owl:Class,
        dcat:Resource ;
    rdfs:label "Item - I93 85  Levy year Collection Act s 41 definition of levy year"@en-AU ;
    dct:isPartOf F1998B00137:91 ;
    dct:isReferencedBy F1998B00137: ;
    rdfs:comment "85  Levy year Collection Act s 41 definition of levy year - Abrievated Graph Key: I93"@en-AU ;
    skos:definition "85  Levy year Collection Act s 41 definition of levy year"@en-AU ;
    skos:narrower F1998B00137:91 ;
    skos:prefLabel "Item I93"@en-AU ;
    dcat:accessURL <https://www.legislation.gov.au/F1998B00137/2024-07-06/2024-07-06/text/original/epub/OEBPS/document_1/document_1.html#_Toc171769326> ;
    dcat:landingPage "https://www.legislation.gov.au/F1998B00137/2024-07-06/2024-07-06/text/original/epub/OEBPS/document_1/document_1.html#_Toc171769326"^^xsd:anyURI ;
    dcat:theme legcons:Item .

F1998B00137:94 a legcons:Item,
        owl:Class,
        dcat:Resource ;
    rdfs:label "Item - I94 86  Producer and proprietor etc of processing establishment are processors for Collection Act"@en-AU ;
    dct:isPartOf F1998B00137:91 ;
    dct:isReferencedBy F1998B00137: ;
    rdfs:comment "86  Producer and proprietor etc of processing establishment are processors for Collection Act - Abrievated Graph Key: I94"@en-AU ;
    skos:definition "86  Producer and proprietor etc of processing establishment are processors for Collection Act"@en-AU ;
    skos:narrower F1998B00137:91 ;
    skos:prefLabel "Item I94"@en-AU ;
    dcat:accessURL <https://www.legislation.gov.au/F1998B00137/2024-07-06/2024-07-06/text/original/epub/OEBPS/document_1/document_1.html#_Toc171769327> ;
    dcat:landingPage "https://www.legislation.gov.au/F1998B00137/2024-07-06/2024-07-06/text/original/epub/OEBPS/document_1/document_1.html#_Toc171769327"^^xsd:anyURI ;
    dcat:theme legcons:Item .

F1998B00137:95 a legcons:Item,
        owl:Class,
        dcat:Resource ;
    rdfs:label "Item - I95 87  Liability of processor as intermediary"@en-AU ;
    dct:isPartOf F1998B00137:91 ;
    dct:isReferencedBy F1998B00137: ;
    rdfs:comment "87  Liability of processor as intermediary - Abrievated Graph Key: I95"@en-AU ;
    skos:definition "87  Liability of processor as intermediary"@en-AU ;
    skos:narrower F1998B00137:91 ;
    skos:prefLabel "Item I95"@en-AU ;
    dcat:accessURL <https://www.legislation.gov.au/F1998B00137/2024-07-06/2024-07-06/text/original/epub/OEBPS/document_1/document_1.html#_Toc171769328> ;
    dcat:landingPage "https://www.legislation.gov.au/F1998B00137/2024-07-06/2024-07-06/text/original/epub/OEBPS/document_1/document_1.html#_Toc171769328"^^xsd:anyURI ;
    dcat:theme legcons:Item .

F1998B00137:96 a legcons:Item,
        owl:Class,
        dcat:Resource ;
    rdfs:label "Item - I96 88  Rate of NRS excise levy on slaughter of horses NRS Excise Levy Act Schedule 8 clause 2"@en-AU ;
    dct:isPartOf F1998B00137:91 ;
    dct:isReferencedBy F1998B00137: ;
    rdfs:comment "88  Rate of NRS excise levy on slaughter of horses NRS Excise Levy Act Schedule 8 clause 2 - Abrievated Graph Key: I96"@en-AU ;
    skos:definition "88  Rate of NRS excise levy on slaughter of horses NRS Excise Levy Act Schedule 8 clause 2"@en-AU ;
    skos:narrower F1998B00137:91 ;
    skos:prefLabel "Item I96"@en-AU ;
    dcat:accessURL <https://www.legislation.gov.au/F1998B00137/2024-07-06/2024-07-06/text/original/epub/OEBPS/document_1/document_1.html#_Toc171769329> ;
    dcat:landingPage "https://www.legislation.gov.au/F1998B00137/2024-07-06/2024-07-06/text/original/epub/OEBPS/document_1/document_1.html#_Toc171769329"^^xsd:anyURI ;
    dcat:theme legcons:Item .

F1998B00137:97 a legcons:Item,
        owl:Class,
        dcat:Resource ;
    rdfs:label "Item - I97 89  When levy is due for payment Collection Act s 6"@en-AU ;
    dct:isPartOf F1998B00137:91 ;
    dct:isReferencedBy F1998B00137: ;
    rdfs:comment "89  When levy is due for payment Collection Act s 6 - Abrievated Graph Key: I97"@en-AU ;
    skos:definition "89  When levy is due for payment Collection Act s 6"@en-AU ;
    skos:narrower F1998B00137:91 ;
    skos:prefLabel "Item I97"@en-AU ;
    dcat:accessURL <https://www.legislation.gov.au/F1998B00137/2024-07-06/2024-07-06/text/original/epub/OEBPS/document_1/document_1.html#_Toc171769330> ;
    dcat:landingPage "https://www.legislation.gov.au/F1998B00137/2024-07-06/2024-07-06/text/original/epub/OEBPS/document_1/document_1.html#_Toc171769330"^^xsd:anyURI ;
    dcat:theme legcons:Item .

F1998B00137:98 a legcons:Item,
        owl:Class,
        dcat:Resource ;
    rdfs:label "Item - I98 90  Owner of carcase is producer for Collection Act"@en-AU ;
    dct:isPartOf F1998B00137:91 ;
    dct:isReferencedBy F1998B00137: ;
    rdfs:comment "90  Owner of carcase is producer for Collection Act - Abrievated Graph Key: I98"@en-AU ;
    skos:definition "90  Owner of carcase is producer for Collection Act"@en-AU ;
    skos:narrower F1998B00137:91 ;
    skos:prefLabel "Item I98"@en-AU ;
    dcat:accessURL <https://www.legislation.gov.au/F1998B00137/2024-07-06/2024-07-06/text/original/epub/OEBPS/document_1/document_1.html#_Toc171769331> ;
    dcat:landingPage "https://www.legislation.gov.au/F1998B00137/2024-07-06/2024-07-06/text/original/epub/OEBPS/document_1/document_1.html#_Toc171769331"^^xsd:anyURI ;
    dcat:theme legcons:Item .

F1998B00137:99 a legcons:Item,
        owl:Class,
        dcat:Resource ;
    rdfs:label "Item - I99 91  Who must give Secretary return"@en-AU ;
    dct:isPartOf F1998B00137:91 ;
    dct:isReferencedBy F1998B00137: ;
    rdfs:comment "91  Who must give Secretary return - Abrievated Graph Key: I99"@en-AU ;
    skos:definition "91  Who must give Secretary return"@en-AU ;
    skos:narrower F1998B00137:91 ;
    skos:prefLabel "Item I99"@en-AU ;
    dcat:accessURL <https://www.legislation.gov.au/F1998B00137/2024-07-06/2024-07-06/text/original/epub/OEBPS/document_1/document_1.html#_Toc171769332> ;
    dcat:landingPage "https://www.legislation.gov.au/F1998B00137/2024-07-06/2024-07-06/text/original/epub/OEBPS/document_1/document_1.html#_Toc171769332"^^xsd:anyURI ;
    dcat:theme legcons:Item .

F1998B00137:106 a legcons:Division,
        owl:Class,
        dcat:Resource ;
    rdfs:label "Division - D106 Division 1 Preliminary"@en-AU ;
    dct:hasPart F1998B00137:107 ;
    dct:isPartOf F1998B00137:105 ;
    dct:isReferencedBy F1998B00137: ;
    rdfs:comment "Division 1 Preliminary - Abrievated Graph Key: D106"@en-AU ;
    skos:broader F1998B00137:107 ;
    skos:definition "Division 1 Preliminary"@en-AU ;
    skos:narrower F1998B00137:105 ;
    skos:prefLabel "Division D106"@en-AU ;
    dcat:accessURL <https://www.legislation.gov.au/F1998B00137/2024-07-06/2024-07-06/text/original/epub/OEBPS/document_1/document_1.html#_Toc171769339> ;
    dcat:landingPage "https://www.legislation.gov.au/F1998B00137/2024-07-06/2024-07-06/text/original/epub/OEBPS/document_1/document_1.html#_Toc171769339"^^xsd:anyURI ;
    dcat:theme legcons:Division .

F1998B00137:177 a legcons:Division,
        owl:Class,
        dcat:Resource ;
    rdfs:label "Division - D177 Division 1 Preliminary"@en-AU ;
    dct:hasPart F1998B00137:178 ;
    dct:isPartOf F1998B00137:176 ;
    dct:isReferencedBy F1998B00137: ;
    rdfs:comment "Division 1 Preliminary - Abrievated Graph Key: D177"@en-AU ;
    skos:broader F1998B00137:178 ;
    skos:definition "Division 1 Preliminary"@en-AU ;
    skos:narrower F1998B00137:176 ;
    skos:prefLabel "Division D177"@en-AU ;
    dcat:accessURL <https://www.legislation.gov.au/F1998B00137/2024-07-06/2024-07-06/text/original/epub/OEBPS/document_1/document_1.html#_Toc171769410> ;
    dcat:landingPage "https://www.legislation.gov.au/F1998B00137/2024-07-06/2024-07-06/text/original/epub/OEBPS/document_1/document_1.html#_Toc171769410"^^xsd:anyURI ;
    dcat:theme legcons:Division .

F1998B00137:1 a legcons:Part,
        owl:Class,
        dcat:Resource ;
    rdfs:label "Part - P1 Part 1 Preliminary"@en-AU ;
    dct:hasPart F1998B00137:2,
        F1998B00137:3,
        F1998B00137:4,
        F1998B00137:5 ;
    dct:isReferencedBy F1998B00137: ;
    rdfs:comment "Part 1 Preliminary - Abrievated Graph Key: P1"@en-AU ;
    skos:broader F1998B00137:2,
        F1998B00137:3,
        F1998B00137:4,
        F1998B00137:5 ;
    skos:definition "Part 1 Preliminary"@en-AU ;
    skos:prefLabel "Part P1"@en-AU ;
    dcat:accessURL <https://www.legislation.gov.au/F1998B00137/2024-07-06/2024-07-06/text/original/epub/OEBPS/document_1/document_1.html#_Toc171769234> ;
    dcat:landingPage "https://www.legislation.gov.au/F1998B00137/2024-07-06/2024-07-06/text/original/epub/OEBPS/document_1/document_1.html#_Toc171769234"^^xsd:anyURI ;
    dcat:theme legcons:Part .

F1998B00137:176 a legcons:Part,
        owl:Class,
        dcat:Resource ;
    rdfs:label "Part - P176 Part 13 Levy on livestock slaughter"@en-AU ;
    dct:hasPart F1998B00137:177,
        F1998B00137:179,
        F1998B00137:186,
        F1998B00137:194 ;
    dct:isReferencedBy F1998B00137: ;
    rdfs:comment "Part 13 Levy on livestock slaughter - Abrievated Graph Key: P176"@en-AU ;
    skos:broader F1998B00137:177,
        F1998B00137:179,
        F1998B00137:186,
        F1998B00137:194 ;
    skos:definition "Part 13 Levy on livestock slaughter"@en-AU ;
    skos:prefLabel "Part P176"@en-AU ;
    dcat:accessURL <https://www.legislation.gov.au/F1998B00137/2024-07-06/2024-07-06/text/original/epub/OEBPS/document_1/document_1.html#_Toc171769409> ;
    dcat:landingPage "https://www.legislation.gov.au/F1998B00137/2024-07-06/2024-07-06/text/original/epub/OEBPS/document_1/document_1.html#_Toc171769409"^^xsd:anyURI ;
    dcat:theme legcons:Part .

F1998B00137:170 a legcons:Part,
        owl:Class,
        dcat:Resource ;
    rdfs:label "Part - P170 Part 12 Levy on laying chickens"@en-AU ;
    dct:hasPart F1998B00137:171,
        F1998B00137:172,
        F1998B00137:173,
        F1998B00137:174,
        F1998B00137:175 ;
    dct:isReferencedBy F1998B00137: ;
    rdfs:comment "Part 12 Levy on laying chickens - Abrievated Graph Key: P170"@en-AU ;
    skos:broader F1998B00137:171,
        F1998B00137:172,
        F1998B00137:173,
        F1998B00137:174,
        F1998B00137:175 ;
    skos:definition "Part 12 Levy on laying chickens"@en-AU ;
    skos:prefLabel "Part P170"@en-AU ;
    dcat:accessURL <https://www.legislation.gov.au/F1998B00137/2024-07-06/2024-07-06/text/original/epub/OEBPS/document_1/document_1.html#_Toc171769403> ;
    dcat:landingPage "https://www.legislation.gov.au/F1998B00137/2024-07-06/2024-07-06/text/original/epub/OEBPS/document_1/document_1.html#_Toc171769403"^^xsd:anyURI ;
    dcat:theme legcons:Part .

F1998B00137:201 a legcons:Part,
        owl:Class,
        dcat:Resource ;
    rdfs:label "Part - P201 Part 14 Levy on meat chickens"@en-AU ;
    dct:hasPart F1998B00137:202,
        F1998B00137:203,
        F1998B00137:204,
        F1998B00137:205,
        F1998B00137:206 ;
    dct:isReferencedBy F1998B00137: ;
    rdfs:comment "Part 14 Levy on meat chickens - Abrievated Graph Key: P201"@en-AU ;
    skos:broader F1998B00137:202,
        F1998B00137:203,
        F1998B00137:204,
        F1998B00137:205,
        F1998B00137:206 ;
    skos:definition "Part 14 Levy on meat chickens"@en-AU ;
    skos:prefLabel "Part P201"@en-AU ;
    dcat:accessURL <https://www.legislation.gov.au/F1998B00137/2024-07-06/2024-07-06/text/original/epub/OEBPS/document_1/document_1.html#_Toc171769434> ;
    dcat:landingPage "https://www.legislation.gov.au/F1998B00137/2024-07-06/2024-07-06/text/original/epub/OEBPS/document_1/document_1.html#_Toc171769434"^^xsd:anyURI ;
    dcat:theme legcons:Part .

F1998B00137:254 a legcons:Endnotes,
        owl:Class,
        dcat:Resource ;
    rdfs:label "Endnotes - E254 Endnotes"@en-AU ;
    dct:hasPart F1998B00137:255,
        F1998B00137:256,
        F1998B00137:257,
        F1998B00137:258 ;
    dct:isPartOf F1998B00137:253 ;
    dct:isReferencedBy F1998B00137: ;
    rdfs:comment "Endnotes - Abrievated Graph Key: E254"@en-AU ;
    skos:broader F1998B00137:255,
        F1998B00137:256,
        F1998B00137:257,
        F1998B00137:258 ;
    skos:definition "Endnotes"@en-AU ;
    skos:narrower F1998B00137:253 ;
    skos:prefLabel "Endnotes E254"@en-AU ;
    dcat:accessURL <https://www.legislation.gov.au/F1998B00137/2024-07-06/2024-07-06/text/original/epub/OEBPS/document_1/document_1.html#_Toc171769487> ;
    dcat:landingPage "https://www.legislation.gov.au/F1998B00137/2024-07-06/2024-07-06/text/original/epub/OEBPS/document_1/document_1.html#_Toc171769487"^^xsd:anyURI ;
    dcat:theme legcons:Endnotes .

F1998B00137:47 a legcons:Part,
        owl:Class,
        dcat:Resource ;
    rdfs:label "Part - P47 Part 5 Levy on dairy produce"@en-AU ;
    dct:hasPart F1998B00137:48,
        F1998B00137:49,
        F1998B00137:50,
        F1998B00137:51,
        F1998B00137:52 ;
    dct:isReferencedBy F1998B00137: ;
    rdfs:comment "Part 5 Levy on dairy produce - Abrievated Graph Key: P47"@en-AU ;
    skos:broader F1998B00137:48,
        F1998B00137:49,
        F1998B00137:50,
        F1998B00137:51,
        F1998B00137:52 ;
    skos:definition "Part 5 Levy on dairy produce"@en-AU ;
    skos:prefLabel "Part P47"@en-AU ;
    dcat:accessURL <https://www.legislation.gov.au/F1998B00137/2024-07-06/2024-07-06/text/original/epub/OEBPS/document_1/document_1.html#_Toc171769280> ;
    dcat:landingPage "https://www.legislation.gov.au/F1998B00137/2024-07-06/2024-07-06/text/original/epub/OEBPS/document_1/document_1.html#_Toc171769280"^^xsd:anyURI ;
    dcat:theme legcons:Part .

F1998B00137:246 a legcons:Part,
        owl:Class,
        dcat:Resource ;
    rdfs:label "Part - P246 Part 18 Levy on wheat"@en-AU ;
    dct:hasPart F1998B00137:247,
        F1998B00137:248,
        F1998B00137:249,
        F1998B00137:250,
        F1998B00137:251,
        F1998B00137:252 ;
    dct:isReferencedBy F1998B00137: ;
    rdfs:comment "Part 18 Levy on wheat - Abrievated Graph Key: P246"@en-AU ;
    skos:broader F1998B00137:247,
        F1998B00137:248,
        F1998B00137:249,
        F1998B00137:250,
        F1998B00137:251,
        F1998B00137:252 ;
    skos:definition "Part 18 Levy on wheat"@en-AU ;
    skos:prefLabel "Part P246"@en-AU ;
    dcat:accessURL <https://www.legislation.gov.au/F1998B00137/2024-07-06/2024-07-06/text/original/epub/OEBPS/document_1/document_1.html#_Toc171769479> ;
    dcat:landingPage "https://www.legislation.gov.au/F1998B00137/2024-07-06/2024-07-06/text/original/epub/OEBPS/document_1/document_1.html#_Toc171769479"^^xsd:anyURI ;
    dcat:theme legcons:Part .

F1998B00137:179 a legcons:Division,
        owl:Class,
        dcat:Resource ;
    rdfs:label "Division - D179 Division 2 Buffalo"@en-AU ;
    dct:hasPart F1998B00137:180,
        F1998B00137:181,
        F1998B00137:182,
        F1998B00137:183,
        F1998B00137:184,
        F1998B00137:185 ;
    dct:isPartOf F1998B00137:176 ;
    dct:isReferencedBy F1998B00137: ;
    rdfs:comment "Division 2 Buffalo - Abrievated Graph Key: D179"@en-AU ;
    skos:broader F1998B00137:180,
        F1998B00137:181,
        F1998B00137:182,
        F1998B00137:183,
        F1998B00137:184,
        F1998B00137:185 ;
    skos:definition "Division 2 Buffalo"@en-AU ;
    skos:narrower F1998B00137:176 ;
    skos:prefLabel "Division D179"@en-AU ;
    dcat:accessURL <https://www.legislation.gov.au/F1998B00137/2024-07-06/2024-07-06/text/original/epub/OEBPS/document_1/document_1.html#_Toc171769412> ;
    dcat:landingPage "https://www.legislation.gov.au/F1998B00137/2024-07-06/2024-07-06/text/original/epub/OEBPS/document_1/document_1.html#_Toc171769412"^^xsd:anyURI ;
    dcat:theme legcons:Division .

F1998B00137:194 a legcons:Division,
        owl:Class,
        dcat:Resource ;
    rdfs:label "Division - D194 Division 4 Pigs"@en-AU ;
    dct:hasPart F1998B00137:195,
        F1998B00137:196,
        F1998B00137:197,
        F1998B00137:198,
        F1998B00137:199,
        F1998B00137:200 ;
    dct:isPartOf F1998B00137:176 ;
    dct:isReferencedBy F1998B00137: ;
    rdfs:comment "Division 4 Pigs - Abrievated Graph Key: D194"@en-AU ;
    skos:broader F1998B00137:195,
        F1998B00137:196,
        F1998B00137:197,
        F1998B00137:198,
        F1998B00137:199,
        F1998B00137:200 ;
    skos:definition "Division 4 Pigs"@en-AU ;
    skos:narrower F1998B00137:176 ;
    skos:prefLabel "Division D194"@en-AU ;
    dcat:accessURL <https://www.legislation.gov.au/F1998B00137/2024-07-06/2024-07-06/text/original/epub/OEBPS/document_1/document_1.html#_Toc171769427> ;
    dcat:landingPage "https://www.legislation.gov.au/F1998B00137/2024-07-06/2024-07-06/text/original/epub/OEBPS/document_1/document_1.html#_Toc171769427"^^xsd:anyURI ;
    dcat:theme legcons:Division .

F1998B00137:53 a legcons:Part,
        owl:Class,
        dcat:Resource ;
    rdfs:label "Part - P53 Part 6 Levy on dried fruits"@en-AU ;
    dct:hasPart F1998B00137:54,
        F1998B00137:55,
        F1998B00137:56,
        F1998B00137:57,
        F1998B00137:58,
        F1998B00137:59,
        F1998B00137:60 ;
    dct:isReferencedBy F1998B00137: ;
    rdfs:comment "Part 6 Levy on dried fruits - Abrievated Graph Key: P53"@en-AU ;
    skos:broader F1998B00137:54,
        F1998B00137:55,
        F1998B00137:56,
        F1998B00137:57,
        F1998B00137:58,
        F1998B00137:59,
        F1998B00137:60 ;
    skos:definition "Part 6 Levy on dried fruits"@en-AU ;
    skos:prefLabel "Part P53"@en-AU ;
    dcat:accessURL <https://www.legislation.gov.au/F1998B00137/2024-07-06/2024-07-06/text/original/epub/OEBPS/document_1/document_1.html#_Toc171769286> ;
    dcat:landingPage "https://www.legislation.gov.au/F1998B00137/2024-07-06/2024-07-06/text/original/epub/OEBPS/document_1/document_1.html#_Toc171769286"^^xsd:anyURI ;
    dcat:theme legcons:Part .

F1998B00137:186 a legcons:Division,
        owl:Class,
        dcat:Resource ;
    rdfs:label "Division - D186 Division 3 Deer"@en-AU ;
    dct:hasPart F1998B00137:187,
        F1998B00137:188,
        F1998B00137:189,
        F1998B00137:190,
        F1998B00137:191,
        F1998B00137:192,
        F1998B00137:193 ;
    dct:isPartOf F1998B00137:176 ;
    dct:isReferencedBy F1998B00137: ;
    rdfs:comment "Division 3 Deer - Abrievated Graph Key: D186"@en-AU ;
    skos:broader F1998B00137:187,
        F1998B00137:188,
        F1998B00137:189,
        F1998B00137:190,
        F1998B00137:191,
        F1998B00137:192,
        F1998B00137:193 ;
    skos:definition "Division 3 Deer"@en-AU ;
    skos:narrower F1998B00137:176 ;
    skos:prefLabel "Division D186"@en-AU ;
    dcat:accessURL <https://www.legislation.gov.au/F1998B00137/2024-07-06/2024-07-06/text/original/epub/OEBPS/document_1/document_1.html#_Toc171769419> ;
    dcat:landingPage "https://www.legislation.gov.au/F1998B00137/2024-07-06/2024-07-06/text/original/epub/OEBPS/document_1/document_1.html#_Toc171769419"^^xsd:anyURI ;
    dcat:theme legcons:Division .

F1998B00137:207 a legcons:Part,
        owl:Class,
        dcat:Resource ;
    rdfs:label "Part - P207 Part 15 Levy on oilseeds"@en-AU ;
    dct:hasPart F1998B00137:208,
        F1998B00137:209,
        F1998B00137:210,
        F1998B00137:211,
        F1998B00137:212,
        F1998B00137:213,
        F1998B00137:214,
        F1998B00137:215 ;
    dct:isReferencedBy F1998B00137: ;
    rdfs:comment "Part 15 Levy on oilseeds - Abrievated Graph Key: P207"@en-AU ;
    skos:broader F1998B00137:208,
        F1998B00137:209,
        F1998B00137:210,
        F1998B00137:211,
        F1998B00137:212,
        F1998B00137:213,
        F1998B00137:214,
        F1998B00137:215 ;
    skos:definition "Part 15 Levy on oilseeds"@en-AU ;
    skos:prefLabel "Part P207"@en-AU ;
    dcat:accessURL <https://www.legislation.gov.au/F1998B00137/2024-07-06/2024-07-06/text/original/epub/OEBPS/document_1/document_1.html#_Toc171769440> ;
    dcat:landingPage "https://www.legislation.gov.au/F1998B00137/2024-07-06/2024-07-06/text/original/epub/OEBPS/document_1/document_1.html#_Toc171769440"^^xsd:anyURI ;
    dcat:theme legcons:Part .

F1998B00137:38 a legcons:Part,
        owl:Class,
        dcat:Resource ;
    rdfs:label "Part - P38 Part 4 Levy on coarse grain"@en-AU ;
    dct:hasPart F1998B00137:39,
        F1998B00137:40,
        F1998B00137:41,
        F1998B00137:42,
        F1998B00137:43,
        F1998B00137:44,
        F1998B00137:45,
        F1998B00137:46 ;
    dct:isReferencedBy F1998B00137: ;
    rdfs:comment "Part 4 Levy on coarse grain - Abrievated Graph Key: P38"@en-AU ;
    skos:broader F1998B00137:39,
        F1998B00137:40,
        F1998B00137:41,
        F1998B00137:42,
        F1998B00137:43,
        F1998B00137:44,
        F1998B00137:45,
        F1998B00137:46 ;
    skos:definition "Part 4 Levy on coarse grain"@en-AU ;
    skos:prefLabel "Part P38"@en-AU ;
    dcat:accessURL <https://www.legislation.gov.au/F1998B00137/2024-07-06/2024-07-06/text/original/epub/OEBPS/document_1/document_1.html#_Toc171769271> ;
    dcat:landingPage "https://www.legislation.gov.au/F1998B00137/2024-07-06/2024-07-06/text/original/epub/OEBPS/document_1/document_1.html#_Toc171769271"^^xsd:anyURI ;
    dcat:theme legcons:Part .

F1998B00137:73 a legcons:Part,
        owl:Class,
        dcat:Resource ;
    rdfs:label "Part - P73 Part 8 Levy on grain legumes"@en-AU ;
    dct:hasPart F1998B00137:74,
        F1998B00137:75,
        F1998B00137:76,
        F1998B00137:77,
        F1998B00137:78,
        F1998B00137:79,
        F1998B00137:80,
        F1998B00137:81 ;
    dct:isReferencedBy F1998B00137: ;
    rdfs:comment "Part 8 Levy on grain legumes - Abrievated Graph Key: P73"@en-AU ;
    skos:broader F1998B00137:74,
        F1998B00137:75,
        F1998B00137:76,
        F1998B00137:77,
        F1998B00137:78,
        F1998B00137:79,
        F1998B00137:80,
        F1998B00137:81 ;
    skos:definition "Part 8 Levy on grain legumes"@en-AU ;
    skos:prefLabel "Part P73"@en-AU ;
    dcat:accessURL <https://www.legislation.gov.au/F1998B00137/2024-07-06/2024-07-06/text/original/epub/OEBPS/document_1/document_1.html#_Toc171769306> ;
    dcat:landingPage "https://www.legislation.gov.au/F1998B00137/2024-07-06/2024-07-06/text/original/epub/OEBPS/document_1/document_1.html#_Toc171769306"^^xsd:anyURI ;
    dcat:theme legcons:Part .

F1998B00137:82 a legcons:Part,
        owl:Class,
        dcat:Resource ;
    rdfs:label "Part - P82 Part 9 Levies on honey and honey export"@en-AU ;
    dct:hasPart F1998B00137:83,
        F1998B00137:84,
        F1998B00137:85,
        F1998B00137:86,
        F1998B00137:87,
        F1998B00137:88,
        F1998B00137:89,
        F1998B00137:90 ;
    dct:isReferencedBy F1998B00137: ;
    rdfs:comment "Part 9 Levies on honey and honey export - Abrievated Graph Key: P82"@en-AU ;
    skos:broader F1998B00137:83,
        F1998B00137:84,
        F1998B00137:85,
        F1998B00137:86,
        F1998B00137:87,
        F1998B00137:88,
        F1998B00137:89,
        F1998B00137:90 ;
    skos:definition "Part 9 Levies on honey and honey export"@en-AU ;
    skos:prefLabel "Part P82"@en-AU ;
    dcat:accessURL <https://www.legislation.gov.au/F1998B00137/2024-07-06/2024-07-06/text/original/epub/OEBPS/document_1/document_1.html#_Toc171769315> ;
    dcat:landingPage "https://www.legislation.gov.au/F1998B00137/2024-07-06/2024-07-06/text/original/epub/OEBPS/document_1/document_1.html#_Toc171769315"^^xsd:anyURI ;
    dcat:theme legcons:Part .

F1998B00137:28 a legcons:Part,
        owl:Class,
        dcat:Resource ;
    rdfs:label "Part - P28 Part 3 Levies on cattle export and cattle transactions"@en-AU ;
    dct:hasPart F1998B00137:29,
        F1998B00137:30,
        F1998B00137:31,
        F1998B00137:32,
        F1998B00137:33,
        F1998B00137:34,
        F1998B00137:35,
        F1998B00137:36,
        F1998B00137:37 ;
    dct:isReferencedBy F1998B00137: ;
    rdfs:comment "Part 3 Levies on cattle export and cattle transactions - Abrievated Graph Key: P28"@en-AU ;
    skos:broader F1998B00137:29,
        F1998B00137:30,
        F1998B00137:31,
        F1998B00137:32,
        F1998B00137:33,
        F1998B00137:34,
        F1998B00137:35,
        F1998B00137:36,
        F1998B00137:37 ;
    skos:definition "Part 3 Levies on cattle export and cattle transactions"@en-AU ;
    skos:prefLabel "Part P28"@en-AU ;
    dcat:accessURL <https://www.legislation.gov.au/F1998B00137/2024-07-06/2024-07-06/text/original/epub/OEBPS/document_1/document_1.html#_Toc171769261> ;
    dcat:landingPage "https://www.legislation.gov.au/F1998B00137/2024-07-06/2024-07-06/text/original/epub/OEBPS/document_1/document_1.html#_Toc171769261"^^xsd:anyURI ;
    dcat:theme legcons:Part .

F1998B00137:61 a legcons:Part,
        owl:Class,
        dcat:Resource ;
    rdfs:label "Part - P61 Part 7 Levy on game animals"@en-AU ;
    dct:hasPart F1998B00137:62,
        F1998B00137:63,
        F1998B00137:64,
        F1998B00137:65,
        F1998B00137:66,
        F1998B00137:67,
        F1998B00137:68,
        F1998B00137:69,
        F1998B00137:70,
        F1998B00137:71,
        F1998B00137:72 ;
    dct:isReferencedBy F1998B00137: ;
    rdfs:comment "Part 7 Levy on game animals - Abrievated Graph Key: P61"@en-AU ;
    skos:broader F1998B00137:62,
        F1998B00137:63,
        F1998B00137:64,
        F1998B00137:65,
        F1998B00137:66,
        F1998B00137:67,
        F1998B00137:68,
        F1998B00137:69,
        F1998B00137:70,
        F1998B00137:71,
        F1998B00137:72 ;
    skos:definition "Part 7 Levy on game animals"@en-AU ;
    skos:prefLabel "Part P61"@en-AU ;
    dcat:accessURL <https://www.legislation.gov.au/F1998B00137/2024-07-06/2024-07-06/text/original/epub/OEBPS/document_1/document_1.html#_Toc171769294> ;
    dcat:landingPage "https://www.legislation.gov.au/F1998B00137/2024-07-06/2024-07-06/text/original/epub/OEBPS/document_1/document_1.html#_Toc171769294"^^xsd:anyURI ;
    dcat:theme legcons:Part .

F1998B00137:91 a legcons:Part,
        owl:Class,
        dcat:Resource ;
    rdfs:label "Part - P91 Part 10 Levy on horse slaughter"@en-AU ;
    dct:hasPart F1998B00137:100,
        F1998B00137:101,
        F1998B00137:102,
        F1998B00137:103,
        F1998B00137:104,
        F1998B00137:92,
        F1998B00137:93,
        F1998B00137:94,
        F1998B00137:95,
        F1998B00137:96,
        F1998B00137:97,
        F1998B00137:98,
        F1998B00137:99 ;
    dct:isReferencedBy F1998B00137: ;
    rdfs:comment "Part 10 Levy on horse slaughter - Abrievated Graph Key: P91"@en-AU ;
    skos:broader F1998B00137:100,
        F1998B00137:101,
        F1998B00137:102,
        F1998B00137:103,
        F1998B00137:104,
        F1998B00137:92,
        F1998B00137:93,
        F1998B00137:94,
        F1998B00137:95,
        F1998B00137:96,
        F1998B00137:97,
        F1998B00137:98,
        F1998B00137:99 ;
    skos:definition "Part 10 Levy on horse slaughter"@en-AU ;
    skos:prefLabel "Part P91"@en-AU ;
    dcat:accessURL <https://www.legislation.gov.au/F1998B00137/2024-07-06/2024-07-06/text/original/epub/OEBPS/document_1/document_1.html#_Toc171769324> ;
    dcat:landingPage "https://www.legislation.gov.au/F1998B00137/2024-07-06/2024-07-06/text/original/epub/OEBPS/document_1/document_1.html#_Toc171769324"^^xsd:anyURI ;
    dcat:theme legcons:Part .

F1998B00137:216 a legcons:Part,
        owl:Class,
        dcat:Resource ;
    rdfs:label "Part - P216 Part 16 Levy on ratite slaughter"@en-AU ;
    dct:hasPart F1998B00137:217,
        F1998B00137:218,
        F1998B00137:219,
        F1998B00137:220,
        F1998B00137:221,
        F1998B00137:222,
        F1998B00137:223,
        F1998B00137:224,
        F1998B00137:225,
        F1998B00137:226,
        F1998B00137:227,
        F1998B00137:228,
        F1998B00137:229,
        F1998B00137:230 ;
    dct:isReferencedBy F1998B00137: ;
    rdfs:comment "Part 16 Levy on ratite slaughter - Abrievated Graph Key: P216"@en-AU ;
    skos:broader F1998B00137:217,
        F1998B00137:218,
        F1998B00137:219,
        F1998B00137:220,
        F1998B00137:221,
        F1998B00137:222,
        F1998B00137:223,
        F1998B00137:224,
        F1998B00137:225,
        F1998B00137:226,
        F1998B00137:227,
        F1998B00137:228,
        F1998B00137:229,
        F1998B00137:230 ;
    skos:definition "Part 16 Levy on ratite slaughter"@en-AU ;
    skos:prefLabel "Part P216"@en-AU ;
    dcat:accessURL <https://www.legislation.gov.au/F1998B00137/2024-07-06/2024-07-06/text/original/epub/OEBPS/document_1/document_1.html#_Toc171769449> ;
    dcat:landingPage "https://www.legislation.gov.au/F1998B00137/2024-07-06/2024-07-06/text/original/epub/OEBPS/document_1/document_1.html#_Toc171769449"^^xsd:anyURI ;
    dcat:theme legcons:Part .

F1998B00137:231 a legcons:Part,
        owl:Class,
        dcat:Resource ;
    rdfs:label "Part - P231 Part 17 Levies on sheep lambs and goats transactions etc and sheep lambs and goats export"@en-AU ;
    dct:hasPart F1998B00137:232,
        F1998B00137:233,
        F1998B00137:234,
        F1998B00137:235,
        F1998B00137:236,
        F1998B00137:237,
        F1998B00137:238,
        F1998B00137:239,
        F1998B00137:240,
        F1998B00137:241,
        F1998B00137:242,
        F1998B00137:243,
        F1998B00137:244,
        F1998B00137:245 ;
    dct:isReferencedBy F1998B00137: ;
    rdfs:comment "Part 17 Levies on sheep lambs and goats transactions etc and sheep lambs and goats export - Abrievated Graph Key: P231"@en-AU ;
    skos:broader F1998B00137:232,
        F1998B00137:233,
        F1998B00137:234,
        F1998B00137:235,
        F1998B00137:236,
        F1998B00137:237,
        F1998B00137:238,
        F1998B00137:239,
        F1998B00137:240,
        F1998B00137:241,
        F1998B00137:242,
        F1998B00137:243,
        F1998B00137:244,
        F1998B00137:245 ;
    skos:definition "Part 17 Levies on sheep lambs and goats transactions etc and sheep lambs and goats export"@en-AU ;
    skos:prefLabel "Part P231"@en-AU ;
    dcat:accessURL <https://www.legislation.gov.au/F1998B00137/2024-07-06/2024-07-06/text/original/epub/OEBPS/document_1/document_1.html#_Toc171769464> ;
    dcat:landingPage "https://www.legislation.gov.au/F1998B00137/2024-07-06/2024-07-06/text/original/epub/OEBPS/document_1/document_1.html#_Toc171769464"^^xsd:anyURI ;
    dcat:theme legcons:Part .

F1998B00137:6 a legcons:Part,
        owl:Class,
        dcat:Resource ;
    rdfs:label "Part - P6 Part 2 Levy on export of aquatic animals and aquatic animal products"@en-AU ;
    dct:hasPart F1998B00137:10,
        F1998B00137:11,
        F1998B00137:12,
        F1998B00137:13,
        F1998B00137:14,
        F1998B00137:15,
        F1998B00137:16,
        F1998B00137:17,
        F1998B00137:18,
        F1998B00137:19,
        F1998B00137:20,
        F1998B00137:21,
        F1998B00137:22,
        F1998B00137:23,
        F1998B00137:24,
        F1998B00137:25,
        F1998B00137:26,
        F1998B00137:27,
        F1998B00137:7,
        F1998B00137:8,
        F1998B00137:9 ;
    dct:isReferencedBy F1998B00137: ;
    rdfs:comment "Part 2 Levy on export of aquatic animals and aquatic animal products - Abrievated Graph Key: P6"@en-AU ;
    skos:broader F1998B00137:10,
        F1998B00137:11,
        F1998B00137:12,
        F1998B00137:13,
        F1998B00137:14,
        F1998B00137:15,
        F1998B00137:16,
        F1998B00137:17,
        F1998B00137:18,
        F1998B00137:19,
        F1998B00137:20,
        F1998B00137:21,
        F1998B00137:22,
        F1998B00137:23,
        F1998B00137:24,
        F1998B00137:25,
        F1998B00137:26,
        F1998B00137:27,
        F1998B00137:7,
        F1998B00137:8,
        F1998B00137:9 ;
    skos:definition "Part 2 Levy on export of aquatic animals and aquatic animal products"@en-AU ;
    skos:prefLabel "Part P6"@en-AU ;
    dcat:accessURL <https://www.legislation.gov.au/F1998B00137/2024-07-06/2024-07-06/text/original/epub/OEBPS/document_1/document_1.html#_Toc171769239> ;
    dcat:landingPage "https://www.legislation.gov.au/F1998B00137/2024-07-06/2024-07-06/text/original/epub/OEBPS/document_1/document_1.html#_Toc171769239"^^xsd:anyURI ;
    dcat:theme legcons:Part .

F1998B00137:105 a legcons:Part,
        owl:Class,
        dcat:Resource ;
    rdfs:label "Part - P105 Part 11 Levies on horticultural products and horticultural products export"@en-AU ;
    dct:hasPart F1998B00137:106,
        F1998B00137:108,
        F1998B00137:109,
        F1998B00137:110,
        F1998B00137:111,
        F1998B00137:112,
        F1998B00137:113,
        F1998B00137:114,
        F1998B00137:115,
        F1998B00137:116,
        F1998B00137:117,
        F1998B00137:118,
        F1998B00137:119,
        F1998B00137:120,
        F1998B00137:121,
        F1998B00137:122,
        F1998B00137:123,
        F1998B00137:124,
        F1998B00137:125,
        F1998B00137:126,
        F1998B00137:127,
        F1998B00137:128,
        F1998B00137:129,
        F1998B00137:130,
        F1998B00137:131,
        F1998B00137:132,
        F1998B00137:133,
        F1998B00137:134,
        F1998B00137:135,
        F1998B00137:136,
        F1998B00137:137,
        F1998B00137:138,
        F1998B00137:139,
        F1998B00137:140,
        F1998B00137:141,
        F1998B00137:142,
        F1998B00137:143,
        F1998B00137:144,
        F1998B00137:145,
        F1998B00137:146,
        F1998B00137:147,
        F1998B00137:148,
        F1998B00137:149,
        F1998B00137:150,
        F1998B00137:151,
        F1998B00137:152,
        F1998B00137:153,
        F1998B00137:154,
        F1998B00137:155,
        F1998B00137:156,
        F1998B00137:157,
        F1998B00137:158,
        F1998B00137:159,
        F1998B00137:160,
        F1998B00137:161,
        F1998B00137:162,
        F1998B00137:163,
        F1998B00137:164,
        F1998B00137:165,
        F1998B00137:166,
        F1998B00137:167,
        F1998B00137:168,
        F1998B00137:169 ;
    dct:isReferencedBy F1998B00137: ;
    rdfs:comment "Part 11 Levies on horticultural products and horticultural products export - Abrievated Graph Key: P105"@en-AU ;
    skos:broader F1998B00137:106,
        F1998B00137:108,
        F1998B00137:109,
        F1998B00137:110,
        F1998B00137:111,
        F1998B00137:112,
        F1998B00137:113,
        F1998B00137:114,
        F1998B00137:115,
        F1998B00137:116,
        F1998B00137:117,
        F1998B00137:118,
        F1998B00137:119,
        F1998B00137:120,
        F1998B00137:121,
        F1998B00137:122,
        F1998B00137:123,
        F1998B00137:124,
        F1998B00137:125,
        F1998B00137:126,
        F1998B00137:127,
        F1998B00137:128,
        F1998B00137:129,
        F1998B00137:130,
        F1998B00137:131,
        F1998B00137:132,
        F1998B00137:133,
        F1998B00137:134,
        F1998B00137:135,
        F1998B00137:136,
        F1998B00137:137,
        F1998B00137:138,
        F1998B00137:139,
        F1998B00137:140,
        F1998B00137:141,
        F1998B00137:142,
        F1998B00137:143,
        F1998B00137:144,
        F1998B00137:145,
        F1998B00137:146,
        F1998B00137:147,
        F1998B00137:148,
        F1998B00137:149,
        F1998B00137:150,
        F1998B00137:151,
        F1998B00137:152,
        F1998B00137:153,
        F1998B00137:154,
        F1998B00137:155,
        F1998B00137:156,
        F1998B00137:157,
        F1998B00137:158,
        F1998B00137:159,
        F1998B00137:160,
        F1998B00137:161,
        F1998B00137:162,
        F1998B00137:163,
        F1998B00137:164,
        F1998B00137:165,
        F1998B00137:166,
        F1998B00137:167,
        F1998B00137:168,
        F1998B00137:169 ;
    skos:definition "Part 11 Levies on horticultural products and horticultural products export"@en-AU ;
    skos:prefLabel "Part P105"@en-AU ;
    dcat:accessURL <https://www.legislation.gov.au/F1998B00137/2024-07-06/2024-07-06/text/original/epub/OEBPS/document_1/document_1.html#_Toc171769338> ;
    dcat:landingPage "https://www.legislation.gov.au/F1998B00137/2024-07-06/2024-07-06/text/original/epub/OEBPS/document_1/document_1.html#_Toc171769338"^^xsd:anyURI ;
    dcat:theme legcons:Part .

F1998B00137: a owl:Class,
        dcat:Dataset,
        dcat:Resource ;
    rdfs:label "Primary Industries Levies and Charges (National Residue Survey Levies) Regulations 1998" ;
    dct:Jurisdiction " Department of Agriculture, Fisheries and Forestry "@en-AU ;
    dct:created "2024-08-30T15:23:31.310447"^^xsd:dateTime ;
    dct:creator "https://orcid.org/0009-0007-8434-7325"^^xsd:anyURI ;
    dct:date "2024-07-06T00:00:00+10:00"^^xsd:dateTime ;
    dct:description "Primary Industries Levies and Charges (National Residue Survey Levies) Regulations 1998"@en-AU ;
    dct:identifier "https://www.legislation.gov.au/F1998B00137/latest"^^xsd:anyURI ;
    dct:license <https://creativecommons.org/licenses/by-sa/4.0/> ;
    dct:source "scheme=AGLSTERMS.AglsAgent; corporateName=Office Parliamentary Counsel; address=Locked Bag 30 Kingston ACT 2604; contact=+61 2 6120 1400"@en-AU ;
    dct:subject "Primary Industries Levies and Charges (National Residue Survey Levies) Regulations 1998"@en-AU ;
    dct:title "Primary Industries Levies and Charges (National Residue Survey Levies) Regulations 1998"@en-AU ;
    owl:imports legcons: ;
    dcat:theme legcons:Division,
        legcons:Endnotes,
        legcons:Item,
        legcons:Part,
        legcons:Schedule ;
    schema:identifier "F1998B00137" ;
    schema:status "In force" ;
    schema:version "F2024C00610 (C39)" .

