@prefix F2021L00315: <http://example.org/au/leg/dataset/F2021L00315/> .
@prefix dcat: <http://www.w3.org/ns/dcat#> .
@prefix dct: <http://purl.org/dc/terms/> .
@prefix legcons: <http://example.org/au/leg/concepts/> .
@prefix owl: <http://www.w3.org/2002/07/owl#> .
@prefix rdfs: <http://www.w3.org/2000/01/rdf-schema#> .
@prefix schema: <https://schema.org/> .
@prefix skos: <http://www.w3.org/2004/02/skos/core#> .
@prefix xsd: <http://www.w3.org/2001/XMLSchema#> .

F2021L00315:10 a legcons:Item,
        owl:Class,
        dcat:Resource ;
    rdfs:label "Item - I10 1 8  Meaning of small horticultural products registered establishment"@en-AU ;
    dct:isPartOf F2021L00315:1 ;
    dct:isReferencedBy F2021L00315: ;
    rdfs:comment "1 8  Meaning of small horticultural products registered establishment - Abrievated Graph Key: I10"@en-AU ;
    skos:definition "1 8  Meaning of small horticultural products registered establishment"@en-AU ;
    skos:narrower F2021L00315:1 ;
    skos:prefLabel "Item I10"@en-AU ;
    dcat:accessURL <https://www.legislation.gov.au/F2021L00315/2023-08-04/2023-08-04/text/original/epub/OEBPS/document_1/document_1.html#_Toc143853834> ;
    dcat:landingPage "https://www.legislation.gov.au/F2021L00315/2023-08-04/2023-08-04/text/original/epub/OEBPS/document_1/document_1.html#_Toc143853834"^^xsd:anyURI ;
    dcat:theme legcons:Item .

F2021L00315:101 a legcons:Item,
        owl:Class,
        dcat:Resource ;
    rdfs:label "Item - I101 4 20  Information to be included in request to revoke registration"@en-AU ;
    dct:isPartOf F2021L00315:100 ;
    dct:isReferencedBy F2021L00315: ;
    rdfs:comment "4 20  Information to be included in request to revoke registration - Abrievated Graph Key: I101"@en-AU ;
    skos:definition "4 20  Information to be included in request to revoke registration"@en-AU ;
    skos:narrower F2021L00315:100 ;
    skos:prefLabel "Item I101"@en-AU ;
    dcat:accessURL <https://www.legislation.gov.au/F2021L00315/2023-08-04/2023-08-04/text/original/epub/OEBPS/document_1/document_1.html#_Toc143853925> ;
    dcat:landingPage "https://www.legislation.gov.au/F2021L00315/2023-08-04/2023-08-04/text/original/epub/OEBPS/document_1/document_1.html#_Toc143853925"^^xsd:anyURI ;
    dcat:theme legcons:Item .

F2021L00315:103 a legcons:Item,
        owl:Class,
        dcat:Resource ;
    rdfs:label "Item - I103 4 21  Other grounds for revocation of registration"@en-AU ;
    dct:isPartOf F2021L00315:102 ;
    dct:isReferencedBy F2021L00315: ;
    rdfs:comment "4 21  Other grounds for revocation of registration - Abrievated Graph Key: I103"@en-AU ;
    skos:definition "4 21  Other grounds for revocation of registration"@en-AU ;
    skos:narrower F2021L00315:102 ;
    skos:prefLabel "Item I103"@en-AU ;
    dcat:accessURL <https://www.legislation.gov.au/F2021L00315/2023-08-04/2023-08-04/text/original/epub/OEBPS/document_1/document_1.html#_Toc143853927> ;
    dcat:landingPage "https://www.legislation.gov.au/F2021L00315/2023-08-04/2023-08-04/text/original/epub/OEBPS/document_1/document_1.html#_Toc143853927"^^xsd:anyURI ;
    dcat:theme legcons:Item .

F2021L00315:105 a legcons:Item,
        owl:Class,
        dcat:Resource ;
    rdfs:label "Item - I105 4 22  Changes in relation to registered establishment that was being treated as small horticultural products registered establishment for a financial year"@en-AU ;
    dct:isPartOf F2021L00315:104 ;
    dct:isReferencedBy F2021L00315: ;
    rdfs:comment "4 22  Changes in relation to registered establishment that was being treated as small horticultural products registered establishment for a financial year - Abrievated Graph Key: I105"@en-AU ;
    skos:definition "4 22  Changes in relation to registered establishment that was being treated as small horticultural products registered establishment for a financial year"@en-AU ;
    skos:narrower F2021L00315:104 ;
    skos:prefLabel "Item I105"@en-AU ;
    dcat:accessURL <https://www.legislation.gov.au/F2021L00315/2023-08-04/2023-08-04/text/original/epub/OEBPS/document_1/document_1.html#_Toc143853929> ;
    dcat:landingPage "https://www.legislation.gov.au/F2021L00315/2023-08-04/2023-08-04/text/original/epub/OEBPS/document_1/document_1.html#_Toc143853929"^^xsd:anyURI ;
    dcat:theme legcons:Item .

F2021L00315:107 a legcons:Item,
        owl:Class,
        dcat:Resource ;
    rdfs:label "Item - I107 4 23  Application of this Part"@en-AU ;
    dct:isPartOf F2021L00315:106 ;
    dct:isReferencedBy F2021L00315: ;
    rdfs:comment "4 23  Application of this Part - Abrievated Graph Key: I107"@en-AU ;
    skos:definition "4 23  Application of this Part"@en-AU ;
    skos:narrower F2021L00315:106 ;
    skos:prefLabel "Item I107"@en-AU ;
    dcat:accessURL <https://www.legislation.gov.au/F2021L00315/2023-08-04/2023-08-04/text/original/epub/OEBPS/document_1/document_1.html#_Toc143853931> ;
    dcat:landingPage "https://www.legislation.gov.au/F2021L00315/2023-08-04/2023-08-04/text/original/epub/OEBPS/document_1/document_1.html#_Toc143853931"^^xsd:anyURI ;
    dcat:theme legcons:Item .

F2021L00315:108 a legcons:Item,
        owl:Class,
        dcat:Resource ;
    rdfs:label "Item - I108 4 24  Initial consideration period"@en-AU ;
    dct:isPartOf F2021L00315:106 ;
    dct:isReferencedBy F2021L00315: ;
    rdfs:comment "4 24  Initial consideration period - Abrievated Graph Key: I108"@en-AU ;
    skos:definition "4 24  Initial consideration period"@en-AU ;
    skos:narrower F2021L00315:106 ;
    skos:prefLabel "Item I108"@en-AU ;
    dcat:accessURL <https://www.legislation.gov.au/F2021L00315/2023-08-04/2023-08-04/text/original/epub/OEBPS/document_1/document_1.html#_Toc143853932> ;
    dcat:landingPage "https://www.legislation.gov.au/F2021L00315/2023-08-04/2023-08-04/text/original/epub/OEBPS/document_1/document_1.html#_Toc143853932"^^xsd:anyURI ;
    dcat:theme legcons:Item .

F2021L00315:109 a legcons:Item,
        owl:Class,
        dcat:Resource ;
    rdfs:label "Item - I109 4 25  Period within which request relating to application must be complied with"@en-AU ;
    dct:isPartOf F2021L00315:106 ;
    dct:isReferencedBy F2021L00315: ;
    rdfs:comment "4 25  Period within which request relating to application must be complied with - Abrievated Graph Key: I109"@en-AU ;
    skos:definition "4 25  Period within which request relating to application must be complied with"@en-AU ;
    skos:narrower F2021L00315:106 ;
    skos:prefLabel "Item I109"@en-AU ;
    dcat:accessURL <https://www.legislation.gov.au/F2021L00315/2023-08-04/2023-08-04/text/original/epub/OEBPS/document_1/document_1.html#_Toc143853933> ;
    dcat:landingPage "https://www.legislation.gov.au/F2021L00315/2023-08-04/2023-08-04/text/original/epub/OEBPS/document_1/document_1.html#_Toc143853933"^^xsd:anyURI ;
    dcat:theme legcons:Item .

F2021L00315:112 a legcons:Item,
        owl:Class,
        dcat:Resource ;
    rdfs:label "Item - I112 7 1  Conditions of export permit"@en-AU ;
    dct:isPartOf F2021L00315:111 ;
    dct:isReferencedBy F2021L00315: ;
    rdfs:comment "7 1  Conditions of export permit - Abrievated Graph Key: I112"@en-AU ;
    skos:definition "7 1  Conditions of export permit"@en-AU ;
    skos:narrower F2021L00315:111 ;
    skos:prefLabel "Item I112"@en-AU ;
    dcat:accessURL <https://www.legislation.gov.au/F2021L00315/2023-08-04/2023-08-04/text/original/epub/OEBPS/document_1/document_1.html#_Toc143853936> ;
    dcat:landingPage "https://www.legislation.gov.au/F2021L00315/2023-08-04/2023-08-04/text/original/epub/OEBPS/document_1/document_1.html#_Toc143853936"^^xsd:anyURI ;
    dcat:theme legcons:Item .

F2021L00315:113 a legcons:Item,
        owl:Class,
        dcat:Resource ;
    rdfs:label "Item - I113 7 2  Period of effect of export permit"@en-AU ;
    dct:isPartOf F2021L00315:111 ;
    dct:isReferencedBy F2021L00315: ;
    rdfs:comment "7 2  Period of effect of export permit - Abrievated Graph Key: I113"@en-AU ;
    skos:definition "7 2  Period of effect of export permit"@en-AU ;
    skos:narrower F2021L00315:111 ;
    skos:prefLabel "Item I113"@en-AU ;
    dcat:accessURL <https://www.legislation.gov.au/F2021L00315/2023-08-04/2023-08-04/text/original/epub/OEBPS/document_1/document_1.html#_Toc143853937> ;
    dcat:landingPage "https://www.legislation.gov.au/F2021L00315/2023-08-04/2023-08-04/text/original/epub/OEBPS/document_1/document_1.html#_Toc143853937"^^xsd:anyURI ;
    dcat:theme legcons:Item .

F2021L00315:115 a legcons:Item,
        owl:Class,
        dcat:Resource ;
    rdfs:label "Item - I115 7 3  Circumstances for varying export permit or conditions of export permit"@en-AU ;
    dct:isPartOf F2021L00315:114 ;
    dct:isReferencedBy F2021L00315: ;
    rdfs:comment "7 3  Circumstances for varying export permit or conditions of export permit - Abrievated Graph Key: I115"@en-AU ;
    skos:definition "7 3  Circumstances for varying export permit or conditions of export permit"@en-AU ;
    skos:narrower F2021L00315:114 ;
    skos:prefLabel "Item I115"@en-AU ;
    dcat:accessURL <https://www.legislation.gov.au/F2021L00315/2023-08-04/2023-08-04/text/original/epub/OEBPS/document_1/document_1.html#_Toc143853939> ;
    dcat:landingPage "https://www.legislation.gov.au/F2021L00315/2023-08-04/2023-08-04/text/original/epub/OEBPS/document_1/document_1.html#_Toc143853939"^^xsd:anyURI ;
    dcat:theme legcons:Item .

F2021L00315:116 a legcons:Item,
        owl:Class,
        dcat:Resource ;
    rdfs:label "Item - I116 7 4  Period of effect of varied export permit"@en-AU ;
    dct:isPartOf F2021L00315:114 ;
    dct:isReferencedBy F2021L00315: ;
    rdfs:comment "7 4  Period of effect of varied export permit - Abrievated Graph Key: I116"@en-AU ;
    skos:definition "7 4  Period of effect of varied export permit"@en-AU ;
    skos:narrower F2021L00315:114 ;
    skos:prefLabel "Item I116"@en-AU ;
    dcat:accessURL <https://www.legislation.gov.au/F2021L00315/2023-08-04/2023-08-04/text/original/epub/OEBPS/document_1/document_1.html#_Toc143853940> ;
    dcat:landingPage "https://www.legislation.gov.au/F2021L00315/2023-08-04/2023-08-04/text/original/epub/OEBPS/document_1/document_1.html#_Toc143853940"^^xsd:anyURI ;
    dcat:theme legcons:Item .

F2021L00315:117 a legcons:Item,
        owl:Class,
        dcat:Resource ;
    rdfs:label "Item - I117 7 5  Circumstances in which export permit may be suspended"@en-AU ;
    dct:isPartOf F2021L00315:114 ;
    dct:isReferencedBy F2021L00315: ;
    rdfs:comment "7 5  Circumstances in which export permit may be suspended - Abrievated Graph Key: I117"@en-AU ;
    skos:definition "7 5  Circumstances in which export permit may be suspended"@en-AU ;
    skos:narrower F2021L00315:114 ;
    skos:prefLabel "Item I117"@en-AU ;
    dcat:accessURL <https://www.legislation.gov.au/F2021L00315/2023-08-04/2023-08-04/text/original/epub/OEBPS/document_1/document_1.html#_Toc143853941> ;
    dcat:landingPage "https://www.legislation.gov.au/F2021L00315/2023-08-04/2023-08-04/text/original/epub/OEBPS/document_1/document_1.html#_Toc143853941"^^xsd:anyURI ;
    dcat:theme legcons:Item .

F2021L00315:118 a legcons:Item,
        owl:Class,
        dcat:Resource ;
    rdfs:label "Item - I118 7 6  Other circumstances in which export permit may be revoked"@en-AU ;
    dct:isPartOf F2021L00315:114 ;
    dct:isReferencedBy F2021L00315: ;
    rdfs:comment "7 6  Other circumstances in which export permit may be revoked - Abrievated Graph Key: I118"@en-AU ;
    skos:definition "7 6  Other circumstances in which export permit may be revoked"@en-AU ;
    skos:narrower F2021L00315:114 ;
    skos:prefLabel "Item I118"@en-AU ;
    dcat:accessURL <https://www.legislation.gov.au/F2021L00315/2023-08-04/2023-08-04/text/original/epub/OEBPS/document_1/document_1.html#_Toc143853942> ;
    dcat:landingPage "https://www.legislation.gov.au/F2021L00315/2023-08-04/2023-08-04/text/original/epub/OEBPS/document_1/document_1.html#_Toc143853942"^^xsd:anyURI ;
    dcat:theme legcons:Item .

F2021L00315:120 a legcons:Item,
        owl:Class,
        dcat:Resource ;
    rdfs:label "Item - I120 7 7  Other circumstances in which the Secretary may require assessment of prescribed plants or plant products"@en-AU ;
    dct:isPartOf F2021L00315:119 ;
    dct:isReferencedBy F2021L00315: ;
    rdfs:comment "7 7  Other circumstances in which the Secretary may require assessment of prescribed plants or plant products - Abrievated Graph Key: I120"@en-AU ;
    skos:definition "7 7  Other circumstances in which the Secretary may require assessment of prescribed plants or plant products"@en-AU ;
    skos:narrower F2021L00315:119 ;
    skos:prefLabel "Item I120"@en-AU ;
    dcat:accessURL <https://www.legislation.gov.au/F2021L00315/2023-08-04/2023-08-04/text/original/epub/OEBPS/document_1/document_1.html#_Toc143853944> ;
    dcat:landingPage "https://www.legislation.gov.au/F2021L00315/2023-08-04/2023-08-04/text/original/epub/OEBPS/document_1/document_1.html#_Toc143853944"^^xsd:anyURI ;
    dcat:theme legcons:Item .

F2021L00315:121 a legcons:Item,
        owl:Class,
        dcat:Resource ;
    rdfs:label "Item - I121 7 8  Changes that require additional or corrected information to be given to the Secretary"@en-AU ;
    dct:isPartOf F2021L00315:119 ;
    dct:isReferencedBy F2021L00315: ;
    rdfs:comment "7 8  Changes that require additional or corrected information to be given to the Secretary - Abrievated Graph Key: I121"@en-AU ;
    skos:definition "7 8  Changes that require additional or corrected information to be given to the Secretary"@en-AU ;
    skos:narrower F2021L00315:119 ;
    skos:prefLabel "Item I121"@en-AU ;
    dcat:accessURL <https://www.legislation.gov.au/F2021L00315/2023-08-04/2023-08-04/text/original/epub/OEBPS/document_1/document_1.html#_Toc143853945> ;
    dcat:landingPage "https://www.legislation.gov.au/F2021L00315/2023-08-04/2023-08-04/text/original/epub/OEBPS/document_1/document_1.html#_Toc143853945"^^xsd:anyURI ;
    dcat:theme legcons:Item .

F2021L00315:123 a legcons:Item,
        owl:Class,
        dcat:Resource ;
    rdfs:label "Item - I123 7 9  Changes that require additional or corrected information to be given to the Secretary"@en-AU ;
    dct:isPartOf F2021L00315:122 ;
    dct:isReferencedBy F2021L00315: ;
    rdfs:comment "7 9  Changes that require additional or corrected information to be given to the Secretary - Abrievated Graph Key: I123"@en-AU ;
    skos:definition "7 9  Changes that require additional or corrected information to be given to the Secretary"@en-AU ;
    skos:narrower F2021L00315:122 ;
    skos:prefLabel "Item I123"@en-AU ;
    dcat:accessURL <https://www.legislation.gov.au/F2021L00315/2023-08-04/2023-08-04/text/original/epub/OEBPS/document_1/document_1.html#_Toc143853947> ;
    dcat:landingPage "https://www.legislation.gov.au/F2021L00315/2023-08-04/2023-08-04/text/original/epub/OEBPS/document_1/document_1.html#_Toc143853947"^^xsd:anyURI ;
    dcat:theme legcons:Item .

F2021L00315:124 a legcons:Item,
        owl:Class,
        dcat:Resource ;
    rdfs:label "Item - I124 7 10  Other powers of the Secretary in considering applications"@en-AU ;
    dct:isPartOf F2021L00315:122 ;
    dct:isReferencedBy F2021L00315: ;
    rdfs:comment "7 10  Other powers of the Secretary in considering applications - Abrievated Graph Key: I124"@en-AU ;
    skos:definition "7 10  Other powers of the Secretary in considering applications"@en-AU ;
    skos:narrower F2021L00315:122 ;
    skos:prefLabel "Item I124"@en-AU ;
    dcat:accessURL <https://www.legislation.gov.au/F2021L00315/2023-08-04/2023-08-04/text/original/epub/OEBPS/document_1/document_1.html#_Toc143853948> ;
    dcat:landingPage "https://www.legislation.gov.au/F2021L00315/2023-08-04/2023-08-04/text/original/epub/OEBPS/document_1/document_1.html#_Toc143853948"^^xsd:anyURI ;
    dcat:theme legcons:Item .

F2021L00315:127 a legcons:Item,
        owl:Class,
        dcat:Resource ;
    rdfs:label "Item - I127 8 1  Person who must give notice of intention to export"@en-AU ;
    dct:isPartOf F2021L00315:126 ;
    dct:isReferencedBy F2021L00315: ;
    rdfs:comment "8 1  Person who must give notice of intention to export - Abrievated Graph Key: I127"@en-AU ;
    skos:definition "8 1  Person who must give notice of intention to export"@en-AU ;
    skos:narrower F2021L00315:126 ;
    skos:prefLabel "Item I127"@en-AU ;
    dcat:accessURL <https://www.legislation.gov.au/F2021L00315/2023-08-04/2023-08-04/text/original/epub/OEBPS/document_1/document_1.html#_Toc143853951> ;
    dcat:landingPage "https://www.legislation.gov.au/F2021L00315/2023-08-04/2023-08-04/text/original/epub/OEBPS/document_1/document_1.html#_Toc143853951"^^xsd:anyURI ;
    dcat:theme legcons:Item .

F2021L00315:128 a legcons:Item,
        owl:Class,
        dcat:Resource ;
    rdfs:label "Item - I128 8 2  Persons to whom notice of intention to export must be given"@en-AU ;
    dct:isPartOf F2021L00315:126 ;
    dct:isReferencedBy F2021L00315: ;
    rdfs:comment "8 2  Persons to whom notice of intention to export must be given - Abrievated Graph Key: I128"@en-AU ;
    skos:definition "8 2  Persons to whom notice of intention to export must be given"@en-AU ;
    skos:narrower F2021L00315:126 ;
    skos:prefLabel "Item I128"@en-AU ;
    dcat:accessURL <https://www.legislation.gov.au/F2021L00315/2023-08-04/2023-08-04/text/original/epub/OEBPS/document_1/document_1.html#_Toc143853952> ;
    dcat:landingPage "https://www.legislation.gov.au/F2021L00315/2023-08-04/2023-08-04/text/original/epub/OEBPS/document_1/document_1.html#_Toc143853952"^^xsd:anyURI ;
    dcat:theme legcons:Item .

F2021L00315:129 a legcons:Item,
        owl:Class,
        dcat:Resource ;
    rdfs:label "Item - I129 8 3  When notice of intention to export must be given"@en-AU ;
    dct:isPartOf F2021L00315:126 ;
    dct:isReferencedBy F2021L00315: ;
    rdfs:comment "8 3  When notice of intention to export must be given - Abrievated Graph Key: I129"@en-AU ;
    skos:definition "8 3  When notice of intention to export must be given"@en-AU ;
    skos:narrower F2021L00315:126 ;
    skos:prefLabel "Item I129"@en-AU ;
    dcat:accessURL <https://www.legislation.gov.au/F2021L00315/2023-08-04/2023-08-04/text/original/epub/OEBPS/document_1/document_1.html#_Toc143853953> ;
    dcat:landingPage "https://www.legislation.gov.au/F2021L00315/2023-08-04/2023-08-04/text/original/epub/OEBPS/document_1/document_1.html#_Toc143853953"^^xsd:anyURI ;
    dcat:theme legcons:Item .

F2021L00315:130 a legcons:Item,
        owl:Class,
        dcat:Resource ;
    rdfs:label "Item - I130 8 4  Additional or corrected information"@en-AU ;
    dct:isPartOf F2021L00315:126 ;
    dct:isReferencedBy F2021L00315: ;
    rdfs:comment "8 4  Additional or corrected information - Abrievated Graph Key: I130"@en-AU ;
    skos:definition "8 4  Additional or corrected information"@en-AU ;
    skos:narrower F2021L00315:126 ;
    skos:prefLabel "Item I130"@en-AU ;
    dcat:accessURL <https://www.legislation.gov.au/F2021L00315/2023-08-04/2023-08-04/text/original/epub/OEBPS/document_1/document_1.html#_Toc143853954> ;
    dcat:landingPage "https://www.legislation.gov.au/F2021L00315/2023-08-04/2023-08-04/text/original/epub/OEBPS/document_1/document_1.html#_Toc143853954"^^xsd:anyURI ;
    dcat:theme legcons:Item .

F2021L00315:132 a legcons:Item,
        owl:Class,
        dcat:Resource ;
    rdfs:label "Item - I132 8 5  Purpose of this Part"@en-AU ;
    dct:isPartOf F2021L00315:131 ;
    dct:isReferencedBy F2021L00315: ;
    rdfs:comment "8 5  Purpose of this Part - Abrievated Graph Key: I132"@en-AU ;
    skos:definition "8 5  Purpose of this Part"@en-AU ;
    skos:narrower F2021L00315:131 ;
    skos:prefLabel "Item I132"@en-AU ;
    dcat:accessURL <https://www.legislation.gov.au/F2021L00315/2023-08-04/2023-08-04/text/original/epub/OEBPS/document_1/document_1.html#_Toc143853956> ;
    dcat:landingPage "https://www.legislation.gov.au/F2021L00315/2023-08-04/2023-08-04/text/original/epub/OEBPS/document_1/document_1.html#_Toc143853956"^^xsd:anyURI ;
    dcat:theme legcons:Item .

F2021L00315:133 a legcons:Item,
        owl:Class,
        dcat:Resource ;
    rdfs:label "Item - I133 8 6  Trade description must be applied to prescribed plants or plant products that are intended to be exported"@en-AU ;
    dct:isPartOf F2021L00315:131 ;
    dct:isReferencedBy F2021L00315: ;
    rdfs:comment "8 6  Trade description must be applied to prescribed plants or plant products that are intended to be exported - Abrievated Graph Key: I133"@en-AU ;
    skos:definition "8 6  Trade description must be applied to prescribed plants or plant products that are intended to be exported"@en-AU ;
    skos:narrower F2021L00315:131 ;
    skos:prefLabel "Item I133"@en-AU ;
    dcat:accessURL <https://www.legislation.gov.au/F2021L00315/2023-08-04/2023-08-04/text/original/epub/OEBPS/document_1/document_1.html#_Toc143853957> ;
    dcat:landingPage "https://www.legislation.gov.au/F2021L00315/2023-08-04/2023-08-04/text/original/epub/OEBPS/document_1/document_1.html#_Toc143853957"^^xsd:anyURI ;
    dcat:theme legcons:Item .

F2021L00315:134 a legcons:Item,
        owl:Class,
        dcat:Resource ;
    rdfs:label "Item - I134 8 7  General requirements for trade descriptions"@en-AU ;
    dct:isPartOf F2021L00315:131 ;
    dct:isReferencedBy F2021L00315: ;
    rdfs:comment "8 7  General requirements for trade descriptions - Abrievated Graph Key: I134"@en-AU ;
    skos:definition "8 7  General requirements for trade descriptions"@en-AU ;
    skos:narrower F2021L00315:131 ;
    skos:prefLabel "Item I134"@en-AU ;
    dcat:accessURL <https://www.legislation.gov.au/F2021L00315/2023-08-04/2023-08-04/text/original/epub/OEBPS/document_1/document_1.html#_Toc143853958> ;
    dcat:landingPage "https://www.legislation.gov.au/F2021L00315/2023-08-04/2023-08-04/text/original/epub/OEBPS/document_1/document_1.html#_Toc143853958"^^xsd:anyURI ;
    dcat:theme legcons:Item .

F2021L00315:135 a legcons:Item,
        owl:Class,
        dcat:Resource ;
    rdfs:label "Item - I135 8 8  Trade descriptions in language other than English"@en-AU ;
    dct:isPartOf F2021L00315:131 ;
    dct:isReferencedBy F2021L00315: ;
    rdfs:comment "8 8  Trade descriptions in language other than English - Abrievated Graph Key: I135"@en-AU ;
    skos:definition "8 8  Trade descriptions in language other than English"@en-AU ;
    skos:narrower F2021L00315:131 ;
    skos:prefLabel "Item I135"@en-AU ;
    dcat:accessURL <https://www.legislation.gov.au/F2021L00315/2023-08-04/2023-08-04/text/original/epub/OEBPS/document_1/document_1.html#_Toc143853959> ;
    dcat:landingPage "https://www.legislation.gov.au/F2021L00315/2023-08-04/2023-08-04/text/original/epub/OEBPS/document_1/document_1.html#_Toc143853959"^^xsd:anyURI ;
    dcat:theme legcons:Item .

F2021L00315:138 a legcons:Item,
        owl:Class,
        dcat:Resource ;
    rdfs:label "Item - I138 8 9  Purpose of this Division"@en-AU ;
    dct:isPartOf F2021L00315:137 ;
    dct:isReferencedBy F2021L00315: ;
    rdfs:comment "8 9  Purpose of this Division - Abrievated Graph Key: I138"@en-AU ;
    skos:definition "8 9  Purpose of this Division"@en-AU ;
    skos:narrower F2021L00315:137 ;
    skos:prefLabel "Item I138"@en-AU ;
    dcat:accessURL <https://www.legislation.gov.au/F2021L00315/2023-08-04/2023-08-04/text/original/epub/OEBPS/document_1/document_1.html#_Toc143853962> ;
    dcat:landingPage "https://www.legislation.gov.au/F2021L00315/2023-08-04/2023-08-04/text/original/epub/OEBPS/document_1/document_1.html#_Toc143853962"^^xsd:anyURI ;
    dcat:theme legcons:Item .

F2021L00315:139 a legcons:Item,
        owl:Class,
        dcat:Resource ;
    rdfs:label "Item - I139 8 10  Tolerances for dimensions of official marks"@en-AU ;
    dct:isPartOf F2021L00315:137 ;
    dct:isReferencedBy F2021L00315: ;
    rdfs:comment "8 10  Tolerances for dimensions of official marks - Abrievated Graph Key: I139"@en-AU ;
    skos:definition "8 10  Tolerances for dimensions of official marks"@en-AU ;
    skos:narrower F2021L00315:137 ;
    skos:prefLabel "Item I139"@en-AU ;
    dcat:accessURL <https://www.legislation.gov.au/F2021L00315/2023-08-04/2023-08-04/text/original/epub/OEBPS/document_1/document_1.html#_Toc143853963> ;
    dcat:landingPage "https://www.legislation.gov.au/F2021L00315/2023-08-04/2023-08-04/text/original/epub/OEBPS/document_1/document_1.html#_Toc143853963"^^xsd:anyURI ;
    dcat:theme legcons:Item .

F2021L00315:14 a legcons:Item,
        owl:Class,
        dcat:Resource ;
    rdfs:label "Item - I14 2 1  Plants and plant products that are prescribed goods"@en-AU ;
    dct:isPartOf F2021L00315:13 ;
    dct:isReferencedBy F2021L00315: ;
    rdfs:comment "2 1  Plants and plant products that are prescribed goods - Abrievated Graph Key: I14"@en-AU ;
    skos:definition "2 1  Plants and plant products that are prescribed goods"@en-AU ;
    skos:narrower F2021L00315:13 ;
    skos:prefLabel "Item I14"@en-AU ;
    dcat:accessURL <https://www.legislation.gov.au/F2021L00315/2023-08-04/2023-08-04/text/original/epub/OEBPS/document_1/document_1.html#_Toc143853838> ;
    dcat:landingPage "https://www.legislation.gov.au/F2021L00315/2023-08-04/2023-08-04/text/original/epub/OEBPS/document_1/document_1.html#_Toc143853838"^^xsd:anyURI ;
    dcat:theme legcons:Item .

F2021L00315:140 a legcons:Item,
        owl:Class,
        dcat:Resource ;
    rdfs:label "Item - I140 8 11  Official markforeign country identification"@en-AU ;
    dct:isPartOf F2021L00315:137 ;
    dct:isReferencedBy F2021L00315: ;
    rdfs:comment "8 11  Official markforeign country identification - Abrievated Graph Key: I140"@en-AU ;
    skos:definition "8 11  Official markforeign country identification"@en-AU ;
    skos:narrower F2021L00315:137 ;
    skos:prefLabel "Item I140"@en-AU ;
    dcat:accessURL <https://www.legislation.gov.au/F2021L00315/2023-08-04/2023-08-04/text/original/epub/OEBPS/document_1/document_1.html#_Toc143853964> ;
    dcat:landingPage "https://www.legislation.gov.au/F2021L00315/2023-08-04/2023-08-04/text/original/epub/OEBPS/document_1/document_1.html#_Toc143853964"^^xsd:anyURI ;
    dcat:theme legcons:Item .

F2021L00315:141 a legcons:Item,
        owl:Class,
        dcat:Resource ;
    rdfs:label "Item - I141 8 12  Official marktamper indicative metal strap seal"@en-AU ;
    dct:isPartOf F2021L00315:137 ;
    dct:isReferencedBy F2021L00315: ;
    rdfs:comment "8 12  Official marktamper indicative metal strap seal - Abrievated Graph Key: I141"@en-AU ;
    skos:definition "8 12  Official marktamper indicative metal strap seal"@en-AU ;
    skos:narrower F2021L00315:137 ;
    skos:prefLabel "Item I141"@en-AU ;
    dcat:accessURL <https://www.legislation.gov.au/F2021L00315/2023-08-04/2023-08-04/text/original/epub/OEBPS/document_1/document_1.html#_Toc143853965> ;
    dcat:landingPage "https://www.legislation.gov.au/F2021L00315/2023-08-04/2023-08-04/text/original/epub/OEBPS/document_1/document_1.html#_Toc143853965"^^xsd:anyURI ;
    dcat:theme legcons:Item .

F2021L00315:142 a legcons:Item,
        owl:Class,
        dcat:Resource ;
    rdfs:label "Item - I142 8 13  Official markbolt seal"@en-AU ;
    dct:isPartOf F2021L00315:137 ;
    dct:isReferencedBy F2021L00315: ;
    rdfs:comment "8 13  Official markbolt seal - Abrievated Graph Key: I142"@en-AU ;
    skos:definition "8 13  Official markbolt seal"@en-AU ;
    skos:narrower F2021L00315:137 ;
    skos:prefLabel "Item I142"@en-AU ;
    dcat:accessURL <https://www.legislation.gov.au/F2021L00315/2023-08-04/2023-08-04/text/original/epub/OEBPS/document_1/document_1.html#_Toc143853966> ;
    dcat:landingPage "https://www.legislation.gov.au/F2021L00315/2023-08-04/2023-08-04/text/original/epub/OEBPS/document_1/document_1.html#_Toc143853966"^^xsd:anyURI ;
    dcat:theme legcons:Item .

F2021L00315:143 a legcons:Item,
        owl:Class,
        dcat:Resource ;
    rdfs:label "Item - I143 8 14  Official markAustralia approved"@en-AU ;
    dct:isPartOf F2021L00315:137 ;
    dct:isReferencedBy F2021L00315: ;
    rdfs:comment "8 14  Official markAustralia approved - Abrievated Graph Key: I143"@en-AU ;
    skos:definition "8 14  Official markAustralia approved"@en-AU ;
    skos:narrower F2021L00315:137 ;
    skos:prefLabel "Item I143"@en-AU ;
    dcat:accessURL <https://www.legislation.gov.au/F2021L00315/2023-08-04/2023-08-04/text/original/epub/OEBPS/document_1/document_1.html#_Toc143853967> ;
    dcat:landingPage "https://www.legislation.gov.au/F2021L00315/2023-08-04/2023-08-04/text/original/epub/OEBPS/document_1/document_1.html#_Toc143853967"^^xsd:anyURI ;
    dcat:theme legcons:Item .

F2021L00315:144 a legcons:Item,
        owl:Class,
        dcat:Resource ;
    rdfs:label "Item - I144 8 15  Official markapproved for export"@en-AU ;
    dct:isPartOf F2021L00315:137 ;
    dct:isReferencedBy F2021L00315: ;
    rdfs:comment "8 15  Official markapproved for export - Abrievated Graph Key: I144"@en-AU ;
    skos:definition "8 15  Official markapproved for export"@en-AU ;
    skos:narrower F2021L00315:137 ;
    skos:prefLabel "Item I144"@en-AU ;
    dcat:accessURL <https://www.legislation.gov.au/F2021L00315/2023-08-04/2023-08-04/text/original/epub/OEBPS/document_1/document_1.html#_Toc143853968> ;
    dcat:landingPage "https://www.legislation.gov.au/F2021L00315/2023-08-04/2023-08-04/text/original/epub/OEBPS/document_1/document_1.html#_Toc143853968"^^xsd:anyURI ;
    dcat:theme legcons:Item .

F2021L00315:145 a legcons:Item,
        owl:Class,
        dcat:Resource ;
    rdfs:label "Item - I145 8 16  Official markcarton seal"@en-AU ;
    dct:isPartOf F2021L00315:137 ;
    dct:isReferencedBy F2021L00315: ;
    rdfs:comment "8 16  Official markcarton seal - Abrievated Graph Key: I145"@en-AU ;
    skos:definition "8 16  Official markcarton seal"@en-AU ;
    skos:narrower F2021L00315:137 ;
    skos:prefLabel "Item I145"@en-AU ;
    dcat:accessURL <https://www.legislation.gov.au/F2021L00315/2023-08-04/2023-08-04/text/original/epub/OEBPS/document_1/document_1.html#_Toc143853969> ;
    dcat:landingPage "https://www.legislation.gov.au/F2021L00315/2023-08-04/2023-08-04/text/original/epub/OEBPS/document_1/document_1.html#_Toc143853969"^^xsd:anyURI ;
    dcat:theme legcons:Item .

F2021L00315:146 a legcons:Item,
        owl:Class,
        dcat:Resource ;
    rdfs:label "Item - I146 8 17  Official markcarton seal plants or plant products opened for assessment and resealed"@en-AU ;
    dct:isPartOf F2021L00315:137 ;
    dct:isReferencedBy F2021L00315: ;
    rdfs:comment "8 17  Official markcarton seal plants or plant products opened for assessment and resealed - Abrievated Graph Key: I146"@en-AU ;
    skos:definition "8 17  Official markcarton seal plants or plant products opened for assessment and resealed"@en-AU ;
    skos:narrower F2021L00315:137 ;
    skos:prefLabel "Item I146"@en-AU ;
    dcat:accessURL <https://www.legislation.gov.au/F2021L00315/2023-08-04/2023-08-04/text/original/epub/OEBPS/document_1/document_1.html#_Toc143853970> ;
    dcat:landingPage "https://www.legislation.gov.au/F2021L00315/2023-08-04/2023-08-04/text/original/epub/OEBPS/document_1/document_1.html#_Toc143853970"^^xsd:anyURI ;
    dcat:theme legcons:Item .

F2021L00315:147 a legcons:Item,
        owl:Class,
        dcat:Resource ;
    rdfs:label "Item - I147 8 18  Official markAustralian Government"@en-AU ;
    dct:isPartOf F2021L00315:137 ;
    dct:isReferencedBy F2021L00315: ;
    rdfs:comment "8 18  Official markAustralian Government - Abrievated Graph Key: I147"@en-AU ;
    skos:definition "8 18  Official markAustralian Government"@en-AU ;
    skos:narrower F2021L00315:137 ;
    skos:prefLabel "Item I147"@en-AU ;
    dcat:accessURL <https://www.legislation.gov.au/F2021L00315/2023-08-04/2023-08-04/text/original/epub/OEBPS/document_1/document_1.html#_Toc143853971> ;
    dcat:landingPage "https://www.legislation.gov.au/F2021L00315/2023-08-04/2023-08-04/text/original/epub/OEBPS/document_1/document_1.html#_Toc143853971"^^xsd:anyURI ;
    dcat:theme legcons:Item .

F2021L00315:148 a legcons:Item,
        owl:Class,
        dcat:Resource ;
    rdfs:label "Item - I148 8 19  Official markEuropean Union"@en-AU ;
    dct:isPartOf F2021L00315:137 ;
    dct:isReferencedBy F2021L00315: ;
    rdfs:comment "8 19  Official markEuropean Union - Abrievated Graph Key: I148"@en-AU ;
    skos:definition "8 19  Official markEuropean Union"@en-AU ;
    skos:narrower F2021L00315:137 ;
    skos:prefLabel "Item I148"@en-AU ;
    dcat:accessURL <https://www.legislation.gov.au/F2021L00315/2023-08-04/2023-08-04/text/original/epub/OEBPS/document_1/document_1.html#_Toc143853972> ;
    dcat:landingPage "https://www.legislation.gov.au/F2021L00315/2023-08-04/2023-08-04/text/original/epub/OEBPS/document_1/document_1.html#_Toc143853972"^^xsd:anyURI ;
    dcat:theme legcons:Item .

F2021L00315:15 a legcons:Item,
        owl:Class,
        dcat:Resource ;
    rdfs:label "Item - I15 2 2  Plants and plant products that are taken not to be prescribed goods"@en-AU ;
    dct:isPartOf F2021L00315:13 ;
    dct:isReferencedBy F2021L00315: ;
    rdfs:comment "2 2  Plants and plant products that are taken not to be prescribed goods - Abrievated Graph Key: I15"@en-AU ;
    skos:definition "2 2  Plants and plant products that are taken not to be prescribed goods"@en-AU ;
    skos:narrower F2021L00315:13 ;
    skos:prefLabel "Item I15"@en-AU ;
    dcat:accessURL <https://www.legislation.gov.au/F2021L00315/2023-08-04/2023-08-04/text/original/epub/OEBPS/document_1/document_1.html#_Toc143853839> ;
    dcat:landingPage "https://www.legislation.gov.au/F2021L00315/2023-08-04/2023-08-04/text/original/epub/OEBPS/document_1/document_1.html#_Toc143853839"^^xsd:anyURI ;
    dcat:theme legcons:Item .

F2021L00315:150 a legcons:Item,
        owl:Class,
        dcat:Resource ;
    rdfs:label "Item - I150 8 20  Purpose of this Division"@en-AU ;
    dct:isPartOf F2021L00315:149 ;
    dct:isReferencedBy F2021L00315: ;
    rdfs:comment "8 20  Purpose of this Division - Abrievated Graph Key: I150"@en-AU ;
    skos:definition "8 20  Purpose of this Division"@en-AU ;
    skos:narrower F2021L00315:149 ;
    skos:prefLabel "Item I150"@en-AU ;
    dcat:accessURL <https://www.legislation.gov.au/F2021L00315/2023-08-04/2023-08-04/text/original/epub/OEBPS/document_1/document_1.html#_Toc143853974> ;
    dcat:landingPage "https://www.legislation.gov.au/F2021L00315/2023-08-04/2023-08-04/text/original/epub/OEBPS/document_1/document_1.html#_Toc143853974"^^xsd:anyURI ;
    dcat:theme legcons:Item .

F2021L00315:151 a legcons:Item,
        owl:Class,
        dcat:Resource ;
    rdfs:label "Item - I151 8 21  Interpretation"@en-AU ;
    dct:isPartOf F2021L00315:149 ;
    dct:isReferencedBy F2021L00315: ;
    rdfs:comment "8 21  Interpretation - Abrievated Graph Key: I151"@en-AU ;
    skos:definition "8 21  Interpretation"@en-AU ;
    skos:narrower F2021L00315:149 ;
    skos:prefLabel "Item I151"@en-AU ;
    dcat:accessURL <https://www.legislation.gov.au/F2021L00315/2023-08-04/2023-08-04/text/original/epub/OEBPS/document_1/document_1.html#_Toc143853975> ;
    dcat:landingPage "https://www.legislation.gov.au/F2021L00315/2023-08-04/2023-08-04/text/original/epub/OEBPS/document_1/document_1.html#_Toc143853975"^^xsd:anyURI ;
    dcat:theme legcons:Item .

F2021L00315:152 a legcons:Item,
        owl:Class,
        dcat:Resource ;
    rdfs:label "Item - I152 8 22  Persons who may manufacture official marks for plants or plant products"@en-AU ;
    dct:isPartOf F2021L00315:149 ;
    dct:isReferencedBy F2021L00315: ;
    rdfs:comment "8 22  Persons who may manufacture official marks for plants or plant products - Abrievated Graph Key: I152"@en-AU ;
    skos:definition "8 22  Persons who may manufacture official marks for plants or plant products"@en-AU ;
    skos:narrower F2021L00315:149 ;
    skos:prefLabel "Item I152"@en-AU ;
    dcat:accessURL <https://www.legislation.gov.au/F2021L00315/2023-08-04/2023-08-04/text/original/epub/OEBPS/document_1/document_1.html#_Toc143853976> ;
    dcat:landingPage "https://www.legislation.gov.au/F2021L00315/2023-08-04/2023-08-04/text/original/epub/OEBPS/document_1/document_1.html#_Toc143853976"^^xsd:anyURI ;
    dcat:theme legcons:Item .

F2021L00315:153 a legcons:Item,
        owl:Class,
        dcat:Resource ;
    rdfs:label "Item - I153 8 23  Persons who may possess official marks that have not been applied to plants or plant products"@en-AU ;
    dct:isPartOf F2021L00315:149 ;
    dct:isReferencedBy F2021L00315: ;
    rdfs:comment "8 23  Persons who may possess official marks that have not been applied to plants or plant products - Abrievated Graph Key: I153"@en-AU ;
    skos:definition "8 23  Persons who may possess official marks that have not been applied to plants or plant products"@en-AU ;
    skos:narrower F2021L00315:149 ;
    skos:prefLabel "Item I153"@en-AU ;
    dcat:accessURL <https://www.legislation.gov.au/F2021L00315/2023-08-04/2023-08-04/text/original/epub/OEBPS/document_1/document_1.html#_Toc143853977> ;
    dcat:landingPage "https://www.legislation.gov.au/F2021L00315/2023-08-04/2023-08-04/text/original/epub/OEBPS/document_1/document_1.html#_Toc143853977"^^xsd:anyURI ;
    dcat:theme legcons:Item .

F2021L00315:154 a legcons:Item,
        owl:Class,
        dcat:Resource ;
    rdfs:label "Item - I154 8 24  Persons who may apply official marks to plants or plant products"@en-AU ;
    dct:isPartOf F2021L00315:149 ;
    dct:isReferencedBy F2021L00315: ;
    rdfs:comment "8 24  Persons who may apply official marks to plants or plant products - Abrievated Graph Key: I154"@en-AU ;
    skos:definition "8 24  Persons who may apply official marks to plants or plant products"@en-AU ;
    skos:narrower F2021L00315:149 ;
    skos:prefLabel "Item I154"@en-AU ;
    dcat:accessURL <https://www.legislation.gov.au/F2021L00315/2023-08-04/2023-08-04/text/original/epub/OEBPS/document_1/document_1.html#_Toc143853978> ;
    dcat:landingPage "https://www.legislation.gov.au/F2021L00315/2023-08-04/2023-08-04/text/original/epub/OEBPS/document_1/document_1.html#_Toc143853978"^^xsd:anyURI ;
    dcat:theme legcons:Item .

F2021L00315:155 a legcons:Item,
        owl:Class,
        dcat:Resource ;
    rdfs:label "Item - I155 8 25  Alteration of and interference with official marks"@en-AU ;
    dct:isPartOf F2021L00315:149 ;
    dct:isReferencedBy F2021L00315: ;
    rdfs:comment "8 25  Alteration of and interference with official marks - Abrievated Graph Key: I155"@en-AU ;
    skos:definition "8 25  Alteration of and interference with official marks"@en-AU ;
    skos:narrower F2021L00315:149 ;
    skos:prefLabel "Item I155"@en-AU ;
    dcat:accessURL <https://www.legislation.gov.au/F2021L00315/2023-08-04/2023-08-04/text/original/epub/OEBPS/document_1/document_1.html#_Toc143853979> ;
    dcat:landingPage "https://www.legislation.gov.au/F2021L00315/2023-08-04/2023-08-04/text/original/epub/OEBPS/document_1/document_1.html#_Toc143853979"^^xsd:anyURI ;
    dcat:theme legcons:Item .

F2021L00315:156 a legcons:Item,
        owl:Class,
        dcat:Resource ;
    rdfs:label "Item - I156 8 26  Official marks must be legible and securely applied"@en-AU ;
    dct:isPartOf F2021L00315:149 ;
    dct:isReferencedBy F2021L00315: ;
    rdfs:comment "8 26  Official marks must be legible and securely applied - Abrievated Graph Key: I156"@en-AU ;
    skos:definition "8 26  Official marks must be legible and securely applied"@en-AU ;
    skos:narrower F2021L00315:149 ;
    skos:prefLabel "Item I156"@en-AU ;
    dcat:accessURL <https://www.legislation.gov.au/F2021L00315/2023-08-04/2023-08-04/text/original/epub/OEBPS/document_1/document_1.html#_Toc143853980> ;
    dcat:landingPage "https://www.legislation.gov.au/F2021L00315/2023-08-04/2023-08-04/text/original/epub/OEBPS/document_1/document_1.html#_Toc143853980"^^xsd:anyURI ;
    dcat:theme legcons:Item .

F2021L00315:157 a legcons:Item,
        owl:Class,
        dcat:Resource ;
    rdfs:label "Item - I157 8 27  Security of official marks"@en-AU ;
    dct:isPartOf F2021L00315:149 ;
    dct:isReferencedBy F2021L00315: ;
    rdfs:comment "8 27  Security of official marks - Abrievated Graph Key: I157"@en-AU ;
    skos:definition "8 27  Security of official marks"@en-AU ;
    skos:narrower F2021L00315:149 ;
    skos:prefLabel "Item I157"@en-AU ;
    dcat:accessURL <https://www.legislation.gov.au/F2021L00315/2023-08-04/2023-08-04/text/original/epub/OEBPS/document_1/document_1.html#_Toc143853981> ;
    dcat:landingPage "https://www.legislation.gov.au/F2021L00315/2023-08-04/2023-08-04/text/original/epub/OEBPS/document_1/document_1.html#_Toc143853981"^^xsd:anyURI ;
    dcat:theme legcons:Item .

F2021L00315:158 a legcons:Item,
        owl:Class,
        dcat:Resource ;
    rdfs:label "Item - I158 8 28  Removal or defacement of official marks"@en-AU ;
    dct:isPartOf F2021L00315:149 ;
    dct:isReferencedBy F2021L00315: ;
    rdfs:comment "8 28  Removal or defacement of official marks - Abrievated Graph Key: I158"@en-AU ;
    skos:definition "8 28  Removal or defacement of official marks"@en-AU ;
    skos:narrower F2021L00315:149 ;
    skos:prefLabel "Item I158"@en-AU ;
    dcat:accessURL <https://www.legislation.gov.au/F2021L00315/2023-08-04/2023-08-04/text/original/epub/OEBPS/document_1/document_1.html#_Toc143853982> ;
    dcat:landingPage "https://www.legislation.gov.au/F2021L00315/2023-08-04/2023-08-04/text/original/epub/OEBPS/document_1/document_1.html#_Toc143853982"^^xsd:anyURI ;
    dcat:theme legcons:Item .

F2021L00315:159 a legcons:Item,
        owl:Class,
        dcat:Resource ;
    rdfs:label "Item - I159 8 29  Records of official marks manufactured"@en-AU ;
    dct:isPartOf F2021L00315:149 ;
    dct:isReferencedBy F2021L00315: ;
    rdfs:comment "8 29  Records of official marks manufactured - Abrievated Graph Key: I159"@en-AU ;
    skos:definition "8 29  Records of official marks manufactured"@en-AU ;
    skos:narrower F2021L00315:149 ;
    skos:prefLabel "Item I159"@en-AU ;
    dcat:accessURL <https://www.legislation.gov.au/F2021L00315/2023-08-04/2023-08-04/text/original/epub/OEBPS/document_1/document_1.html#_Toc143853983> ;
    dcat:landingPage "https://www.legislation.gov.au/F2021L00315/2023-08-04/2023-08-04/text/original/epub/OEBPS/document_1/document_1.html#_Toc143853983"^^xsd:anyURI ;
    dcat:theme legcons:Item .

F2021L00315:16 a legcons:Division,
        owl:Class,
        dcat:Resource ;
    rdfs:label "Division - D16 Division 2 Prohibited export and prescribed export conditions"@en-AU ;
    dct:isPartOf F2021L00315:12 ;
    dct:isReferencedBy F2021L00315: ;
    rdfs:comment "Division 2 Prohibited export and prescribed export conditions - Abrievated Graph Key: D16"@en-AU ;
    skos:definition "Division 2 Prohibited export and prescribed export conditions"@en-AU ;
    skos:narrower F2021L00315:12 ;
    skos:prefLabel "Division D16"@en-AU ;
    dcat:accessURL <https://www.legislation.gov.au/F2021L00315/2023-08-04/2023-08-04/text/original/epub/OEBPS/document_1/document_1.html#_Toc143853840> ;
    dcat:landingPage "https://www.legislation.gov.au/F2021L00315/2023-08-04/2023-08-04/text/original/epub/OEBPS/document_1/document_1.html#_Toc143853840"^^xsd:anyURI ;
    dcat:theme legcons:Division .

F2021L00315:160 a legcons:Item,
        owl:Class,
        dcat:Resource ;
    rdfs:label "Item - I160 8 30  Records of official marks applied removed defaced destroyed or returned"@en-AU ;
    dct:isPartOf F2021L00315:149 ;
    dct:isReferencedBy F2021L00315: ;
    rdfs:comment "8 30  Records of official marks applied removed defaced destroyed or returned - Abrievated Graph Key: I160"@en-AU ;
    skos:definition "8 30  Records of official marks applied removed defaced destroyed or returned"@en-AU ;
    skos:narrower F2021L00315:149 ;
    skos:prefLabel "Item I160"@en-AU ;
    dcat:accessURL <https://www.legislation.gov.au/F2021L00315/2023-08-04/2023-08-04/text/original/epub/OEBPS/document_1/document_1.html#_Toc143853984> ;
    dcat:landingPage "https://www.legislation.gov.au/F2021L00315/2023-08-04/2023-08-04/text/original/epub/OEBPS/document_1/document_1.html#_Toc143853984"^^xsd:anyURI ;
    dcat:theme legcons:Item .

F2021L00315:162 a legcons:Item,
        owl:Class,
        dcat:Resource ;
    rdfs:label "Item - I162 8 31  Purpose of this Division"@en-AU ;
    dct:isPartOf F2021L00315:161 ;
    dct:isReferencedBy F2021L00315: ;
    rdfs:comment "8 31  Purpose of this Division - Abrievated Graph Key: I162"@en-AU ;
    skos:definition "8 31  Purpose of this Division"@en-AU ;
    skos:narrower F2021L00315:161 ;
    skos:prefLabel "Item I162"@en-AU ;
    dcat:accessURL <https://www.legislation.gov.au/F2021L00315/2023-08-04/2023-08-04/text/original/epub/OEBPS/document_1/document_1.html#_Toc143853986> ;
    dcat:landingPage "https://www.legislation.gov.au/F2021L00315/2023-08-04/2023-08-04/text/original/epub/OEBPS/document_1/document_1.html#_Toc143853986"^^xsd:anyURI ;
    dcat:theme legcons:Item .

F2021L00315:163 a legcons:Item,
        owl:Class,
        dcat:Resource ;
    rdfs:label "Item - I163 8 32  Persons who may manufacture or possess official marking devices"@en-AU ;
    dct:isPartOf F2021L00315:161 ;
    dct:isReferencedBy F2021L00315: ;
    rdfs:comment "8 32  Persons who may manufacture or possess official marking devices - Abrievated Graph Key: I163"@en-AU ;
    skos:definition "8 32  Persons who may manufacture or possess official marking devices"@en-AU ;
    skos:narrower F2021L00315:161 ;
    skos:prefLabel "Item I163"@en-AU ;
    dcat:accessURL <https://www.legislation.gov.au/F2021L00315/2023-08-04/2023-08-04/text/original/epub/OEBPS/document_1/document_1.html#_Toc143853987> ;
    dcat:landingPage "https://www.legislation.gov.au/F2021L00315/2023-08-04/2023-08-04/text/original/epub/OEBPS/document_1/document_1.html#_Toc143853987"^^xsd:anyURI ;
    dcat:theme legcons:Item .

F2021L00315:164 a legcons:Item,
        owl:Class,
        dcat:Resource ;
    rdfs:label "Item - I164 8 33  Security of official marking devices"@en-AU ;
    dct:isPartOf F2021L00315:161 ;
    dct:isReferencedBy F2021L00315: ;
    rdfs:comment "8 33  Security of official marking devices - Abrievated Graph Key: I164"@en-AU ;
    skos:definition "8 33  Security of official marking devices"@en-AU ;
    skos:narrower F2021L00315:161 ;
    skos:prefLabel "Item I164"@en-AU ;
    dcat:accessURL <https://www.legislation.gov.au/F2021L00315/2023-08-04/2023-08-04/text/original/epub/OEBPS/document_1/document_1.html#_Toc143853988> ;
    dcat:landingPage "https://www.legislation.gov.au/F2021L00315/2023-08-04/2023-08-04/text/original/epub/OEBPS/document_1/document_1.html#_Toc143853988"^^xsd:anyURI ;
    dcat:theme legcons:Item .

F2021L00315:165 a legcons:Item,
        owl:Class,
        dcat:Resource ;
    rdfs:label "Item - I165 8 34  Damaged official marking devices"@en-AU ;
    dct:isPartOf F2021L00315:161 ;
    dct:isReferencedBy F2021L00315: ;
    rdfs:comment "8 34  Damaged official marking devices - Abrievated Graph Key: I165"@en-AU ;
    skos:definition "8 34  Damaged official marking devices"@en-AU ;
    skos:narrower F2021L00315:161 ;
    skos:prefLabel "Item I165"@en-AU ;
    dcat:accessURL <https://www.legislation.gov.au/F2021L00315/2023-08-04/2023-08-04/text/original/epub/OEBPS/document_1/document_1.html#_Toc143853989> ;
    dcat:landingPage "https://www.legislation.gov.au/F2021L00315/2023-08-04/2023-08-04/text/original/epub/OEBPS/document_1/document_1.html#_Toc143853989"^^xsd:anyURI ;
    dcat:theme legcons:Item .

F2021L00315:166 a legcons:Item,
        owl:Class,
        dcat:Resource ;
    rdfs:label "Item - I166 8 35  Records of official marking devices manufactured"@en-AU ;
    dct:isPartOf F2021L00315:161 ;
    dct:isReferencedBy F2021L00315: ;
    rdfs:comment "8 35  Records of official marking devices manufactured - Abrievated Graph Key: I166"@en-AU ;
    skos:definition "8 35  Records of official marking devices manufactured"@en-AU ;
    skos:narrower F2021L00315:161 ;
    skos:prefLabel "Item I166"@en-AU ;
    dcat:accessURL <https://www.legislation.gov.au/F2021L00315/2023-08-04/2023-08-04/text/original/epub/OEBPS/document_1/document_1.html#_Toc143853990> ;
    dcat:landingPage "https://www.legislation.gov.au/F2021L00315/2023-08-04/2023-08-04/text/original/epub/OEBPS/document_1/document_1.html#_Toc143853990"^^xsd:anyURI ;
    dcat:theme legcons:Item .

F2021L00315:167 a legcons:Item,
        owl:Class,
        dcat:Resource ;
    rdfs:label "Item - I167 8 36  Records of official marking devices used destroyed or returned"@en-AU ;
    dct:isPartOf F2021L00315:161 ;
    dct:isReferencedBy F2021L00315: ;
    rdfs:comment "8 36  Records of official marking devices used destroyed or returned - Abrievated Graph Key: I167"@en-AU ;
    skos:definition "8 36  Records of official marking devices used destroyed or returned"@en-AU ;
    skos:narrower F2021L00315:161 ;
    skos:prefLabel "Item I167"@en-AU ;
    dcat:accessURL <https://www.legislation.gov.au/F2021L00315/2023-08-04/2023-08-04/text/original/epub/OEBPS/document_1/document_1.html#_Toc143853991> ;
    dcat:landingPage "https://www.legislation.gov.au/F2021L00315/2023-08-04/2023-08-04/text/original/epub/OEBPS/document_1/document_1.html#_Toc143853991"^^xsd:anyURI ;
    dcat:theme legcons:Item .

F2021L00315:17 a legcons:Item,
        owl:Class,
        dcat:Resource ;
    rdfs:label "Item - I17 2 3  Purpose and application of this Division"@en-AU ;
    dct:isPartOf F2021L00315:12 ;
    dct:isReferencedBy F2021L00315: ;
    rdfs:comment "2 3  Purpose and application of this Division - Abrievated Graph Key: I17"@en-AU ;
    skos:definition "2 3  Purpose and application of this Division"@en-AU ;
    skos:narrower F2021L00315:12 ;
    skos:prefLabel "Item I17"@en-AU ;
    dcat:accessURL <https://www.legislation.gov.au/F2021L00315/2023-08-04/2023-08-04/text/original/epub/OEBPS/document_1/document_1.html#_Toc143853841> ;
    dcat:landingPage "https://www.legislation.gov.au/F2021L00315/2023-08-04/2023-08-04/text/original/epub/OEBPS/document_1/document_1.html#_Toc143853841"^^xsd:anyURI ;
    dcat:theme legcons:Item .

F2021L00315:171 a legcons:Item,
        owl:Class,
        dcat:Resource ;
    rdfs:label "Item - I171 9 1  References to audit in this Part"@en-AU ;
    dct:isPartOf F2021L00315:170 ;
    dct:isReferencedBy F2021L00315: ;
    rdfs:comment "9 1  References to audit in this Part - Abrievated Graph Key: I171"@en-AU ;
    skos:definition "9 1  References to audit in this Part"@en-AU ;
    skos:narrower F2021L00315:170 ;
    skos:prefLabel "Item I171"@en-AU ;
    dcat:accessURL <https://www.legislation.gov.au/F2021L00315/2023-08-04/2023-08-04/text/original/epub/OEBPS/document_1/document_1.html#_Toc143853995> ;
    dcat:landingPage "https://www.legislation.gov.au/F2021L00315/2023-08-04/2023-08-04/text/original/epub/OEBPS/document_1/document_1.html#_Toc143853995"^^xsd:anyURI ;
    dcat:theme legcons:Item .

F2021L00315:172 a legcons:Item,
        owl:Class,
        dcat:Resource ;
    rdfs:label "Item - I172 9 2  Other circumstances in which audit of export operations may be required"@en-AU ;
    dct:isPartOf F2021L00315:170 ;
    dct:isReferencedBy F2021L00315: ;
    rdfs:comment "9 2  Other circumstances in which audit of export operations may be required - Abrievated Graph Key: I172"@en-AU ;
    skos:definition "9 2  Other circumstances in which audit of export operations may be required"@en-AU ;
    skos:narrower F2021L00315:170 ;
    skos:prefLabel "Item I172"@en-AU ;
    dcat:accessURL <https://www.legislation.gov.au/F2021L00315/2023-08-04/2023-08-04/text/original/epub/OEBPS/document_1/document_1.html#_Toc143853996> ;
    dcat:landingPage "https://www.legislation.gov.au/F2021L00315/2023-08-04/2023-08-04/text/original/epub/OEBPS/document_1/document_1.html#_Toc143853996"^^xsd:anyURI ;
    dcat:theme legcons:Item .

F2021L00315:174 a legcons:Item,
        owl:Class,
        dcat:Resource ;
    rdfs:label "Item - I174 9 3  Purpose of this Division"@en-AU ;
    dct:isPartOf F2021L00315:173 ;
    dct:isReferencedBy F2021L00315: ;
    rdfs:comment "9 3  Purpose of this Division - Abrievated Graph Key: I174"@en-AU ;
    skos:definition "9 3  Purpose of this Division"@en-AU ;
    skos:narrower F2021L00315:173 ;
    skos:prefLabel "Item I174"@en-AU ;
    dcat:accessURL <https://www.legislation.gov.au/F2021L00315/2023-08-04/2023-08-04/text/original/epub/OEBPS/document_1/document_1.html#_Toc143853998> ;
    dcat:landingPage "https://www.legislation.gov.au/F2021L00315/2023-08-04/2023-08-04/text/original/epub/OEBPS/document_1/document_1.html#_Toc143853998"^^xsd:anyURI ;
    dcat:theme legcons:Item .

F2021L00315:175 a legcons:Item,
        owl:Class,
        dcat:Resource ;
    rdfs:label "Item - I175 9 4  Audit reports"@en-AU ;
    dct:isPartOf F2021L00315:173 ;
    dct:isReferencedBy F2021L00315: ;
    rdfs:comment "9 4  Audit reports - Abrievated Graph Key: I175"@en-AU ;
    skos:definition "9 4  Audit reports"@en-AU ;
    skos:narrower F2021L00315:173 ;
    skos:prefLabel "Item I175"@en-AU ;
    dcat:accessURL <https://www.legislation.gov.au/F2021L00315/2023-08-04/2023-08-04/text/original/epub/OEBPS/document_1/document_1.html#_Toc143853999> ;
    dcat:landingPage "https://www.legislation.gov.au/F2021L00315/2023-08-04/2023-08-04/text/original/epub/OEBPS/document_1/document_1.html#_Toc143853999"^^xsd:anyURI ;
    dcat:theme legcons:Item .

F2021L00315:178 a legcons:Item,
        owl:Class,
        dcat:Resource ;
    rdfs:label "Item - I178 9 5  Circumstances in which assessment may be required or permitted"@en-AU ;
    dct:isPartOf F2021L00315:177 ;
    dct:isReferencedBy F2021L00315: ;
    rdfs:comment "9 5  Circumstances in which assessment may be required or permitted - Abrievated Graph Key: I178"@en-AU ;
    skos:definition "9 5  Circumstances in which assessment may be required or permitted"@en-AU ;
    skos:narrower F2021L00315:177 ;
    skos:prefLabel "Item I178"@en-AU ;
    dcat:accessURL <https://www.legislation.gov.au/F2021L00315/2023-08-04/2023-08-04/text/original/epub/OEBPS/document_1/document_1.html#_Toc143854002> ;
    dcat:landingPage "https://www.legislation.gov.au/F2021L00315/2023-08-04/2023-08-04/text/original/epub/OEBPS/document_1/document_1.html#_Toc143854002"^^xsd:anyURI ;
    dcat:theme legcons:Item .

F2021L00315:179 a legcons:Item,
        owl:Class,
        dcat:Resource ;
    rdfs:label "Item - I179 9 6  Relevant person for assessment"@en-AU ;
    dct:isPartOf F2021L00315:177 ;
    dct:isReferencedBy F2021L00315: ;
    rdfs:comment "9 6  Relevant person for assessment - Abrievated Graph Key: I179"@en-AU ;
    skos:definition "9 6  Relevant person for assessment"@en-AU ;
    skos:narrower F2021L00315:177 ;
    skos:prefLabel "Item I179"@en-AU ;
    dcat:accessURL <https://www.legislation.gov.au/F2021L00315/2023-08-04/2023-08-04/text/original/epub/OEBPS/document_1/document_1.html#_Toc143854003> ;
    dcat:landingPage "https://www.legislation.gov.au/F2021L00315/2023-08-04/2023-08-04/text/original/epub/OEBPS/document_1/document_1.html#_Toc143854003"^^xsd:anyURI ;
    dcat:theme legcons:Item .

F2021L00315:18 a legcons:Item,
        owl:Class,
        dcat:Resource ;
    rdfs:label "Item - I18 2 4  Export of prescribed plants or plant products is prohibited unless prescribed conditions are complied with"@en-AU ;
    dct:isPartOf F2021L00315:12 ;
    dct:isReferencedBy F2021L00315: ;
    rdfs:comment "2 4  Export of prescribed plants or plant products is prohibited unless prescribed conditions are complied with - Abrievated Graph Key: I18"@en-AU ;
    skos:definition "2 4  Export of prescribed plants or plant products is prohibited unless prescribed conditions are complied with"@en-AU ;
    skos:narrower F2021L00315:12 ;
    skos:prefLabel "Item I18"@en-AU ;
    dcat:accessURL <https://www.legislation.gov.au/F2021L00315/2023-08-04/2023-08-04/text/original/epub/OEBPS/document_1/document_1.html#_Toc143853842> ;
    dcat:landingPage "https://www.legislation.gov.au/F2021L00315/2023-08-04/2023-08-04/text/original/epub/OEBPS/document_1/document_1.html#_Toc143853842"^^xsd:anyURI ;
    dcat:theme legcons:Item .

F2021L00315:181 a legcons:Item,
        owl:Class,
        dcat:Resource ;
    rdfs:label "Item - I181 9 7  Purpose of this Division"@en-AU ;
    dct:isPartOf F2021L00315:180 ;
    dct:isReferencedBy F2021L00315: ;
    rdfs:comment "9 7  Purpose of this Division - Abrievated Graph Key: I181"@en-AU ;
    skos:definition "9 7  Purpose of this Division"@en-AU ;
    skos:narrower F2021L00315:180 ;
    skos:prefLabel "Item I181"@en-AU ;
    dcat:accessURL <https://www.legislation.gov.au/F2021L00315/2023-08-04/2023-08-04/text/original/epub/OEBPS/document_1/document_1.html#_Toc143854005> ;
    dcat:landingPage "https://www.legislation.gov.au/F2021L00315/2023-08-04/2023-08-04/text/original/epub/OEBPS/document_1/document_1.html#_Toc143854005"^^xsd:anyURI ;
    dcat:theme legcons:Item .

F2021L00315:182 a legcons:Item,
        owl:Class,
        dcat:Resource ;
    rdfs:label "Item - I182 9 8  Assessments of prescribed plants or plant products"@en-AU ;
    dct:isPartOf F2021L00315:180 ;
    dct:isReferencedBy F2021L00315: ;
    rdfs:comment "9 8  Assessments of prescribed plants or plant products - Abrievated Graph Key: I182"@en-AU ;
    skos:definition "9 8  Assessments of prescribed plants or plant products"@en-AU ;
    skos:narrower F2021L00315:180 ;
    skos:prefLabel "Item I182"@en-AU ;
    dcat:accessURL <https://www.legislation.gov.au/F2021L00315/2023-08-04/2023-08-04/text/original/epub/OEBPS/document_1/document_1.html#_Toc143854006> ;
    dcat:landingPage "https://www.legislation.gov.au/F2021L00315/2023-08-04/2023-08-04/text/original/epub/OEBPS/document_1/document_1.html#_Toc143854006"^^xsd:anyURI ;
    dcat:theme legcons:Item .

F2021L00315:183 a legcons:Item,
        owl:Class,
        dcat:Resource ;
    rdfs:label "Item - I183 9 9  Circumstances when bulk vessel approval or container approval must be provided to assessor"@en-AU ;
    dct:isPartOf F2021L00315:180 ;
    dct:isReferencedBy F2021L00315: ;
    rdfs:comment "9 9  Circumstances when bulk vessel approval or container approval must be provided to assessor - Abrievated Graph Key: I183"@en-AU ;
    skos:definition "9 9  Circumstances when bulk vessel approval or container approval must be provided to assessor"@en-AU ;
    skos:narrower F2021L00315:180 ;
    skos:prefLabel "Item I183"@en-AU ;
    dcat:accessURL <https://www.legislation.gov.au/F2021L00315/2023-08-04/2023-08-04/text/original/epub/OEBPS/document_1/document_1.html#_Toc143854007> ;
    dcat:landingPage "https://www.legislation.gov.au/F2021L00315/2023-08-04/2023-08-04/text/original/epub/OEBPS/document_1/document_1.html#_Toc143854007"^^xsd:anyURI ;
    dcat:theme legcons:Item .

F2021L00315:184 a legcons:Item,
        owl:Class,
        dcat:Resource ;
    rdfs:label "Item - I184 9 10  Criteria for deciding whether plants or plant products pass assessment"@en-AU ;
    dct:isPartOf F2021L00315:180 ;
    dct:isReferencedBy F2021L00315: ;
    rdfs:comment "9 10  Criteria for deciding whether plants or plant products pass assessment - Abrievated Graph Key: I184"@en-AU ;
    skos:definition "9 10  Criteria for deciding whether plants or plant products pass assessment"@en-AU ;
    skos:narrower F2021L00315:180 ;
    skos:prefLabel "Item I184"@en-AU ;
    dcat:accessURL <https://www.legislation.gov.au/F2021L00315/2023-08-04/2023-08-04/text/original/epub/OEBPS/document_1/document_1.html#_Toc143854008> ;
    dcat:landingPage "https://www.legislation.gov.au/F2021L00315/2023-08-04/2023-08-04/text/original/epub/OEBPS/document_1/document_1.html#_Toc143854008"^^xsd:anyURI ;
    dcat:theme legcons:Item .

F2021L00315:185 a legcons:Item,
        owl:Class,
        dcat:Resource ;
    rdfs:label "Item - I185 9 11  Reassessment after failed assessment"@en-AU ;
    dct:isPartOf F2021L00315:180 ;
    dct:isReferencedBy F2021L00315: ;
    rdfs:comment "9 11  Reassessment after failed assessment - Abrievated Graph Key: I185"@en-AU ;
    skos:definition "9 11  Reassessment after failed assessment"@en-AU ;
    skos:narrower F2021L00315:180 ;
    skos:prefLabel "Item I185"@en-AU ;
    dcat:accessURL <https://www.legislation.gov.au/F2021L00315/2023-08-04/2023-08-04/text/original/epub/OEBPS/document_1/document_1.html#_Toc143854009> ;
    dcat:landingPage "https://www.legislation.gov.au/F2021L00315/2023-08-04/2023-08-04/text/original/epub/OEBPS/document_1/document_1.html#_Toc143854009"^^xsd:anyURI ;
    dcat:theme legcons:Item .

F2021L00315:186 a legcons:Item,
        owl:Class,
        dcat:Resource ;
    rdfs:label "Item - I186 9 12  Validity period for plants or plant products"@en-AU ;
    dct:isPartOf F2021L00315:180 ;
    dct:isReferencedBy F2021L00315: ;
    rdfs:comment "9 12  Validity period for plants or plant products - Abrievated Graph Key: I186"@en-AU ;
    skos:definition "9 12  Validity period for plants or plant products"@en-AU ;
    skos:narrower F2021L00315:180 ;
    skos:prefLabel "Item I186"@en-AU ;
    dcat:accessURL <https://www.legislation.gov.au/F2021L00315/2023-08-04/2023-08-04/text/original/epub/OEBPS/document_1/document_1.html#_Toc143854010> ;
    dcat:landingPage "https://www.legislation.gov.au/F2021L00315/2023-08-04/2023-08-04/text/original/epub/OEBPS/document_1/document_1.html#_Toc143854010"^^xsd:anyURI ;
    dcat:theme legcons:Item .

F2021L00315:187 a legcons:Item,
        owl:Class,
        dcat:Resource ;
    rdfs:label "Item - I187 9 13  Relevant person for assessment may apply to extend validity period for plants or plant products"@en-AU ;
    dct:isPartOf F2021L00315:180 ;
    dct:isReferencedBy F2021L00315: ;
    rdfs:comment "9 13  Relevant person for assessment may apply to extend validity period for plants or plant products - Abrievated Graph Key: I187"@en-AU ;
    skos:definition "9 13  Relevant person for assessment may apply to extend validity period for plants or plant products"@en-AU ;
    skos:narrower F2021L00315:180 ;
    skos:prefLabel "Item I187"@en-AU ;
    dcat:accessURL <https://www.legislation.gov.au/F2021L00315/2023-08-04/2023-08-04/text/original/epub/OEBPS/document_1/document_1.html#_Toc143854011> ;
    dcat:landingPage "https://www.legislation.gov.au/F2021L00315/2023-08-04/2023-08-04/text/original/epub/OEBPS/document_1/document_1.html#_Toc143854011"^^xsd:anyURI ;
    dcat:theme legcons:Item .

F2021L00315:188 a legcons:Item,
        owl:Class,
        dcat:Resource ;
    rdfs:label "Item - I188 9 14  Record of assessment"@en-AU ;
    dct:isPartOf F2021L00315:180 ;
    dct:isReferencedBy F2021L00315: ;
    rdfs:comment "9 14  Record of assessment - Abrievated Graph Key: I188"@en-AU ;
    skos:definition "9 14  Record of assessment"@en-AU ;
    skos:narrower F2021L00315:180 ;
    skos:prefLabel "Item I188"@en-AU ;
    dcat:accessURL <https://www.legislation.gov.au/F2021L00315/2023-08-04/2023-08-04/text/original/epub/OEBPS/document_1/document_1.html#_Toc143854012> ;
    dcat:landingPage "https://www.legislation.gov.au/F2021L00315/2023-08-04/2023-08-04/text/original/epub/OEBPS/document_1/document_1.html#_Toc143854012"^^xsd:anyURI ;
    dcat:theme legcons:Item .

F2021L00315:189 a legcons:Item,
        owl:Class,
        dcat:Resource ;
    rdfs:label "Item - I189 9 15  Applicable tolerance levels for pests and contaminants"@en-AU ;
    dct:isPartOf F2021L00315:180 ;
    dct:isReferencedBy F2021L00315: ;
    rdfs:comment "9 15  Applicable tolerance levels for pests and contaminants - Abrievated Graph Key: I189"@en-AU ;
    skos:definition "9 15  Applicable tolerance levels for pests and contaminants"@en-AU ;
    skos:narrower F2021L00315:180 ;
    skos:prefLabel "Item I189"@en-AU ;
    dcat:accessURL <https://www.legislation.gov.au/F2021L00315/2023-08-04/2023-08-04/text/original/epub/OEBPS/document_1/document_1.html#_Toc143854013> ;
    dcat:landingPage "https://www.legislation.gov.au/F2021L00315/2023-08-04/2023-08-04/text/original/epub/OEBPS/document_1/document_1.html#_Toc143854013"^^xsd:anyURI ;
    dcat:theme legcons:Item .

F2021L00315:19 a legcons:Part,
        owl:Class,
        dcat:Resource ;
    rdfs:label "Part - P19 Part 2 Exemptions"@en-AU ;
    dct:isPartOf F2021L00315:11 ;
    dct:isReferencedBy F2021L00315: ;
    rdfs:comment "Part 2 Exemptions - Abrievated Graph Key: P19"@en-AU ;
    skos:definition "Part 2 Exemptions"@en-AU ;
    skos:narrower F2021L00315:11 ;
    skos:prefLabel "Part P19"@en-AU ;
    dcat:accessURL <https://www.legislation.gov.au/F2021L00315/2023-08-04/2023-08-04/text/original/epub/OEBPS/document_1/document_1.html#_Toc143853843> ;
    dcat:landingPage "https://www.legislation.gov.au/F2021L00315/2023-08-04/2023-08-04/text/original/epub/OEBPS/document_1/document_1.html#_Toc143853843"^^xsd:anyURI ;
    dcat:theme legcons:Part .

F2021L00315:190 a legcons:Item,
        owl:Class,
        dcat:Resource ;
    rdfs:label "Item - I190 9 16  Approval of tolerance levels for pests and contaminants"@en-AU ;
    dct:isPartOf F2021L00315:180 ;
    dct:isReferencedBy F2021L00315: ;
    rdfs:comment "9 16  Approval of tolerance levels for pests and contaminants - Abrievated Graph Key: I190"@en-AU ;
    skos:definition "9 16  Approval of tolerance levels for pests and contaminants"@en-AU ;
    skos:narrower F2021L00315:180 ;
    skos:prefLabel "Item I190"@en-AU ;
    dcat:accessURL <https://www.legislation.gov.au/F2021L00315/2023-08-04/2023-08-04/text/original/epub/OEBPS/document_1/document_1.html#_Toc143854014> ;
    dcat:landingPage "https://www.legislation.gov.au/F2021L00315/2023-08-04/2023-08-04/text/original/epub/OEBPS/document_1/document_1.html#_Toc143854014"^^xsd:anyURI ;
    dcat:theme legcons:Item .

F2021L00315:192 a legcons:Item,
        owl:Class,
        dcat:Resource ;
    rdfs:label "Item - I192 9 17  Decisions that may be made by operation of computer program"@en-AU ;
    dct:isPartOf F2021L00315:191 ;
    dct:isReferencedBy F2021L00315: ;
    rdfs:comment "9 17  Decisions that may be made by operation of computer program - Abrievated Graph Key: I192"@en-AU ;
    skos:definition "9 17  Decisions that may be made by operation of computer program"@en-AU ;
    skos:narrower F2021L00315:191 ;
    skos:prefLabel "Item I192"@en-AU ;
    dcat:accessURL <https://www.legislation.gov.au/F2021L00315/2023-08-04/2023-08-04/text/original/epub/OEBPS/document_1/document_1.html#_Toc143854016> ;
    dcat:landingPage "https://www.legislation.gov.au/F2021L00315/2023-08-04/2023-08-04/text/original/epub/OEBPS/document_1/document_1.html#_Toc143854016"^^xsd:anyURI ;
    dcat:theme legcons:Item .

F2021L00315:193 a legcons:Item,
        owl:Class,
        dcat:Resource ;
    rdfs:label "Item - I193 9 18  Functions and powers that must not be subdelegated"@en-AU ;
    dct:isPartOf F2021L00315:191 ;
    dct:isReferencedBy F2021L00315: ;
    rdfs:comment "9 18  Functions and powers that must not be subdelegated - Abrievated Graph Key: I193"@en-AU ;
    skos:definition "9 18  Functions and powers that must not be subdelegated"@en-AU ;
    skos:narrower F2021L00315:191 ;
    skos:prefLabel "Item I193"@en-AU ;
    dcat:accessURL <https://www.legislation.gov.au/F2021L00315/2023-08-04/2023-08-04/text/original/epub/OEBPS/document_1/document_1.html#_Toc143854017> ;
    dcat:landingPage "https://www.legislation.gov.au/F2021L00315/2023-08-04/2023-08-04/text/original/epub/OEBPS/document_1/document_1.html#_Toc143854017"^^xsd:anyURI ;
    dcat:theme legcons:Item .

F2021L00315:195 a legcons:Item,
        owl:Class,
        dcat:Resource ;
    rdfs:label "Item - I195 9 19  Third party authorised officers"@en-AU ;
    dct:isPartOf F2021L00315:194 ;
    dct:isReferencedBy F2021L00315: ;
    rdfs:comment "9 19  Third party authorised officers - Abrievated Graph Key: I195"@en-AU ;
    skos:definition "9 19  Third party authorised officers"@en-AU ;
    skos:narrower F2021L00315:194 ;
    skos:prefLabel "Item I195"@en-AU ;
    dcat:accessURL <https://www.legislation.gov.au/F2021L00315/2023-08-04/2023-08-04/text/original/epub/OEBPS/document_1/document_1.html#_Toc143854019> ;
    dcat:landingPage "https://www.legislation.gov.au/F2021L00315/2023-08-04/2023-08-04/text/original/epub/OEBPS/document_1/document_1.html#_Toc143854019"^^xsd:anyURI ;
    dcat:theme legcons:Item .

F2021L00315:196 a legcons:Item,
        owl:Class,
        dcat:Resource ;
    rdfs:label "Item - I196 9 19 A  Condition of authorisationbulk vessel inspections"@en-AU ;
    dct:isPartOf F2021L00315:194 ;
    dct:isReferencedBy F2021L00315: ;
    rdfs:comment "9 19 A  Condition of authorisationbulk vessel inspections - Abrievated Graph Key: I196"@en-AU ;
    skos:definition "9 19 A  Condition of authorisationbulk vessel inspections"@en-AU ;
    skos:narrower F2021L00315:194 ;
    skos:prefLabel "Item I196"@en-AU ;
    dcat:accessURL <https://www.legislation.gov.au/F2021L00315/2023-08-04/2023-08-04/text/original/epub/OEBPS/document_1/document_1.html#_Toc143854020> ;
    dcat:landingPage "https://www.legislation.gov.au/F2021L00315/2023-08-04/2023-08-04/text/original/epub/OEBPS/document_1/document_1.html#_Toc143854020"^^xsd:anyURI ;
    dcat:theme legcons:Item .

F2021L00315:197 a legcons:Item,
        owl:Class,
        dcat:Resource ;
    rdfs:label "Item - I197 9 20  Functions and powers of authorised officersbulk vessel approvals and container approvals"@en-AU ;
    dct:isPartOf F2021L00315:194 ;
    dct:isReferencedBy F2021L00315: ;
    rdfs:comment "9 20  Functions and powers of authorised officersbulk vessel approvals and container approvals - Abrievated Graph Key: I197"@en-AU ;
    skos:definition "9 20  Functions and powers of authorised officersbulk vessel approvals and container approvals"@en-AU ;
    skos:narrower F2021L00315:194 ;
    skos:prefLabel "Item I197"@en-AU ;
    dcat:accessURL <https://www.legislation.gov.au/F2021L00315/2023-08-04/2023-08-04/text/original/epub/OEBPS/document_1/document_1.html#_Toc143854021> ;
    dcat:landingPage "https://www.legislation.gov.au/F2021L00315/2023-08-04/2023-08-04/text/original/epub/OEBPS/document_1/document_1.html#_Toc143854021"^^xsd:anyURI ;
    dcat:theme legcons:Item .

F2021L00315:198 a legcons:Item,
        owl:Class,
        dcat:Resource ;
    rdfs:label "Item - I198 9 21  Directions to deal with non compliance with the Act etc"@en-AU ;
    dct:isPartOf F2021L00315:194 ;
    dct:isReferencedBy F2021L00315: ;
    rdfs:comment "9 21  Directions to deal with non compliance with the Act etc - Abrievated Graph Key: I198"@en-AU ;
    skos:definition "9 21  Directions to deal with non compliance with the Act etc"@en-AU ;
    skos:narrower F2021L00315:194 ;
    skos:prefLabel "Item I198"@en-AU ;
    dcat:accessURL <https://www.legislation.gov.au/F2021L00315/2023-08-04/2023-08-04/text/original/epub/OEBPS/document_1/document_1.html#_Toc143854022> ;
    dcat:landingPage "https://www.legislation.gov.au/F2021L00315/2023-08-04/2023-08-04/text/original/epub/OEBPS/document_1/document_1.html#_Toc143854022"^^xsd:anyURI ;
    dcat:theme legcons:Item .

F2021L00315:2 a legcons:Part,
        owl:Class,
        dcat:Resource ;
    rdfs:label "Part - P2 Part 1 Preliminary"@en-AU ;
    dct:isPartOf F2021L00315:1 ;
    dct:isReferencedBy F2021L00315: ;
    rdfs:comment "Part 1 Preliminary - Abrievated Graph Key: P2"@en-AU ;
    skos:definition "Part 1 Preliminary"@en-AU ;
    skos:narrower F2021L00315:1 ;
    skos:prefLabel "Part P2"@en-AU ;
    dcat:accessURL <https://www.legislation.gov.au/F2021L00315/2023-08-04/2023-08-04/text/original/epub/OEBPS/document_1/document_1.html#_Toc143853826> ;
    dcat:landingPage "https://www.legislation.gov.au/F2021L00315/2023-08-04/2023-08-04/text/original/epub/OEBPS/document_1/document_1.html#_Toc143853826"^^xsd:anyURI ;
    dcat:theme legcons:Part .

F2021L00315:20 a legcons:Item,
        owl:Class,
        dcat:Resource ;
    rdfs:label "Item - I20 2 5  Application of this Part"@en-AU ;
    dct:isPartOf F2021L00315:11 ;
    dct:isReferencedBy F2021L00315: ;
    rdfs:comment "2 5  Application of this Part - Abrievated Graph Key: I20"@en-AU ;
    skos:definition "2 5  Application of this Part"@en-AU ;
    skos:narrower F2021L00315:11 ;
    skos:prefLabel "Item I20"@en-AU ;
    dcat:accessURL <https://www.legislation.gov.au/F2021L00315/2023-08-04/2023-08-04/text/original/epub/OEBPS/document_1/document_1.html#_Toc143853844> ;
    dcat:landingPage "https://www.legislation.gov.au/F2021L00315/2023-08-04/2023-08-04/text/original/epub/OEBPS/document_1/document_1.html#_Toc143853844"^^xsd:anyURI ;
    dcat:theme legcons:Item .

F2021L00315:200 a legcons:Item,
        owl:Class,
        dcat:Resource ;
    rdfs:label "Item - I200 9 22  Authorised officer may approve bulk vessel"@en-AU ;
    dct:isPartOf F2021L00315:199 ;
    dct:isReferencedBy F2021L00315: ;
    rdfs:comment "9 22  Authorised officer may approve bulk vessel - Abrievated Graph Key: I200"@en-AU ;
    skos:definition "9 22  Authorised officer may approve bulk vessel"@en-AU ;
    skos:narrower F2021L00315:199 ;
    skos:prefLabel "Item I200"@en-AU ;
    dcat:accessURL <https://www.legislation.gov.au/F2021L00315/2023-08-04/2023-08-04/text/original/epub/OEBPS/document_1/document_1.html#_Toc143854024> ;
    dcat:landingPage "https://www.legislation.gov.au/F2021L00315/2023-08-04/2023-08-04/text/original/epub/OEBPS/document_1/document_1.html#_Toc143854024"^^xsd:anyURI ;
    dcat:theme legcons:Item .

F2021L00315:201 a legcons:Item,
        owl:Class,
        dcat:Resource ;
    rdfs:label "Item - I201 9 23  Requirements for approval of bulk vessel"@en-AU ;
    dct:isPartOf F2021L00315:199 ;
    dct:isReferencedBy F2021L00315: ;
    rdfs:comment "9 23  Requirements for approval of bulk vessel - Abrievated Graph Key: I201"@en-AU ;
    skos:definition "9 23  Requirements for approval of bulk vessel"@en-AU ;
    skos:narrower F2021L00315:199 ;
    skos:prefLabel "Item I201"@en-AU ;
    dcat:accessURL <https://www.legislation.gov.au/F2021L00315/2023-08-04/2023-08-04/text/original/epub/OEBPS/document_1/document_1.html#_Toc143854025> ;
    dcat:landingPage "https://www.legislation.gov.au/F2021L00315/2023-08-04/2023-08-04/text/original/epub/OEBPS/document_1/document_1.html#_Toc143854025"^^xsd:anyURI ;
    dcat:theme legcons:Item .

F2021L00315:202 a legcons:Item,
        owl:Class,
        dcat:Resource ;
    rdfs:label "Item - I202 9 24  Bulk vessel inspection record"@en-AU ;
    dct:isPartOf F2021L00315:199 ;
    dct:isReferencedBy F2021L00315: ;
    rdfs:comment "9 24  Bulk vessel inspection record - Abrievated Graph Key: I202"@en-AU ;
    skos:definition "9 24  Bulk vessel inspection record"@en-AU ;
    skos:narrower F2021L00315:199 ;
    skos:prefLabel "Item I202"@en-AU ;
    dcat:accessURL <https://www.legislation.gov.au/F2021L00315/2023-08-04/2023-08-04/text/original/epub/OEBPS/document_1/document_1.html#_Toc143854026> ;
    dcat:landingPage "https://www.legislation.gov.au/F2021L00315/2023-08-04/2023-08-04/text/original/epub/OEBPS/document_1/document_1.html#_Toc143854026"^^xsd:anyURI ;
    dcat:theme legcons:Item .

F2021L00315:203 a legcons:Item,
        owl:Class,
        dcat:Resource ;
    rdfs:label "Item - I203 9 25  Period of effect of bulk vessel approval"@en-AU ;
    dct:isPartOf F2021L00315:199 ;
    dct:isReferencedBy F2021L00315: ;
    rdfs:comment "9 25  Period of effect of bulk vessel approval - Abrievated Graph Key: I203"@en-AU ;
    skos:definition "9 25  Period of effect of bulk vessel approval"@en-AU ;
    skos:narrower F2021L00315:199 ;
    skos:prefLabel "Item I203"@en-AU ;
    dcat:accessURL <https://www.legislation.gov.au/F2021L00315/2023-08-04/2023-08-04/text/original/epub/OEBPS/document_1/document_1.html#_Toc143854027> ;
    dcat:landingPage "https://www.legislation.gov.au/F2021L00315/2023-08-04/2023-08-04/text/original/epub/OEBPS/document_1/document_1.html#_Toc143854027"^^xsd:anyURI ;
    dcat:theme legcons:Item .

F2021L00315:204 a legcons:Item,
        owl:Class,
        dcat:Resource ;
    rdfs:label "Item - I204 9 26  Extension of period of effect of bulk vessel approval"@en-AU ;
    dct:isPartOf F2021L00315:199 ;
    dct:isReferencedBy F2021L00315: ;
    rdfs:comment "9 26  Extension of period of effect of bulk vessel approval - Abrievated Graph Key: I204"@en-AU ;
    skos:definition "9 26  Extension of period of effect of bulk vessel approval"@en-AU ;
    skos:narrower F2021L00315:199 ;
    skos:prefLabel "Item I204"@en-AU ;
    dcat:accessURL <https://www.legislation.gov.au/F2021L00315/2023-08-04/2023-08-04/text/original/epub/OEBPS/document_1/document_1.html#_Toc143854028> ;
    dcat:landingPage "https://www.legislation.gov.au/F2021L00315/2023-08-04/2023-08-04/text/original/epub/OEBPS/document_1/document_1.html#_Toc143854028"^^xsd:anyURI ;
    dcat:theme legcons:Item .

F2021L00315:205 a legcons:Item,
        owl:Class,
        dcat:Resource ;
    rdfs:label "Item - I205 9 27  Suspension of bulk vessel approval"@en-AU ;
    dct:isPartOf F2021L00315:199 ;
    dct:isReferencedBy F2021L00315: ;
    rdfs:comment "9 27  Suspension of bulk vessel approval - Abrievated Graph Key: I205"@en-AU ;
    skos:definition "9 27  Suspension of bulk vessel approval"@en-AU ;
    skos:narrower F2021L00315:199 ;
    skos:prefLabel "Item I205"@en-AU ;
    dcat:accessURL <https://www.legislation.gov.au/F2021L00315/2023-08-04/2023-08-04/text/original/epub/OEBPS/document_1/document_1.html#_Toc143854029> ;
    dcat:landingPage "https://www.legislation.gov.au/F2021L00315/2023-08-04/2023-08-04/text/original/epub/OEBPS/document_1/document_1.html#_Toc143854029"^^xsd:anyURI ;
    dcat:theme legcons:Item .

F2021L00315:206 a legcons:Item,
        owl:Class,
        dcat:Resource ;
    rdfs:label "Item - I206 9 28  Revocation of suspension of bulk vessel approval"@en-AU ;
    dct:isPartOf F2021L00315:199 ;
    dct:isReferencedBy F2021L00315: ;
    rdfs:comment "9 28  Revocation of suspension of bulk vessel approval - Abrievated Graph Key: I206"@en-AU ;
    skos:definition "9 28  Revocation of suspension of bulk vessel approval"@en-AU ;
    skos:narrower F2021L00315:199 ;
    skos:prefLabel "Item I206"@en-AU ;
    dcat:accessURL <https://www.legislation.gov.au/F2021L00315/2023-08-04/2023-08-04/text/original/epub/OEBPS/document_1/document_1.html#_Toc143854030> ;
    dcat:landingPage "https://www.legislation.gov.au/F2021L00315/2023-08-04/2023-08-04/text/original/epub/OEBPS/document_1/document_1.html#_Toc143854030"^^xsd:anyURI ;
    dcat:theme legcons:Item .

F2021L00315:207 a legcons:Item,
        owl:Class,
        dcat:Resource ;
    rdfs:label "Item - I207 9 29  Revocation of bulk vessel approval"@en-AU ;
    dct:isPartOf F2021L00315:199 ;
    dct:isReferencedBy F2021L00315: ;
    rdfs:comment "9 29  Revocation of bulk vessel approval - Abrievated Graph Key: I207"@en-AU ;
    skos:definition "9 29  Revocation of bulk vessel approval"@en-AU ;
    skos:narrower F2021L00315:199 ;
    skos:prefLabel "Item I207"@en-AU ;
    dcat:accessURL <https://www.legislation.gov.au/F2021L00315/2023-08-04/2023-08-04/text/original/epub/OEBPS/document_1/document_1.html#_Toc143854031> ;
    dcat:landingPage "https://www.legislation.gov.au/F2021L00315/2023-08-04/2023-08-04/text/original/epub/OEBPS/document_1/document_1.html#_Toc143854031"^^xsd:anyURI ;
    dcat:theme legcons:Item .

F2021L00315:209 a legcons:Item,
        owl:Class,
        dcat:Resource ;
    rdfs:label "Item - I209 9 30  Authorised officer may approve container"@en-AU ;
    dct:isPartOf F2021L00315:208 ;
    dct:isReferencedBy F2021L00315: ;
    rdfs:comment "9 30  Authorised officer may approve container - Abrievated Graph Key: I209"@en-AU ;
    skos:definition "9 30  Authorised officer may approve container"@en-AU ;
    skos:narrower F2021L00315:208 ;
    skos:prefLabel "Item I209"@en-AU ;
    dcat:accessURL <https://www.legislation.gov.au/F2021L00315/2023-08-04/2023-08-04/text/original/epub/OEBPS/document_1/document_1.html#_Toc143854033> ;
    dcat:landingPage "https://www.legislation.gov.au/F2021L00315/2023-08-04/2023-08-04/text/original/epub/OEBPS/document_1/document_1.html#_Toc143854033"^^xsd:anyURI ;
    dcat:theme legcons:Item .

F2021L00315:21 a legcons:Item,
        owl:Class,
        dcat:Resource ;
    rdfs:label "Item - I21 2 6  Period for making application for exemption"@en-AU ;
    dct:isPartOf F2021L00315:11 ;
    dct:isReferencedBy F2021L00315: ;
    rdfs:comment "2 6  Period for making application for exemption - Abrievated Graph Key: I21"@en-AU ;
    skos:definition "2 6  Period for making application for exemption"@en-AU ;
    skos:narrower F2021L00315:11 ;
    skos:prefLabel "Item I21"@en-AU ;
    dcat:accessURL <https://www.legislation.gov.au/F2021L00315/2023-08-04/2023-08-04/text/original/epub/OEBPS/document_1/document_1.html#_Toc143853845> ;
    dcat:landingPage "https://www.legislation.gov.au/F2021L00315/2023-08-04/2023-08-04/text/original/epub/OEBPS/document_1/document_1.html#_Toc143853845"^^xsd:anyURI ;
    dcat:theme legcons:Item .

F2021L00315:210 a legcons:Item,
        owl:Class,
        dcat:Resource ;
    rdfs:label "Item - I210 9 31  Requirements for approval of container"@en-AU ;
    dct:isPartOf F2021L00315:208 ;
    dct:isReferencedBy F2021L00315: ;
    rdfs:comment "9 31  Requirements for approval of container - Abrievated Graph Key: I210"@en-AU ;
    skos:definition "9 31  Requirements for approval of container"@en-AU ;
    skos:narrower F2021L00315:208 ;
    skos:prefLabel "Item I210"@en-AU ;
    dcat:accessURL <https://www.legislation.gov.au/F2021L00315/2023-08-04/2023-08-04/text/original/epub/OEBPS/document_1/document_1.html#_Toc143854034> ;
    dcat:landingPage "https://www.legislation.gov.au/F2021L00315/2023-08-04/2023-08-04/text/original/epub/OEBPS/document_1/document_1.html#_Toc143854034"^^xsd:anyURI ;
    dcat:theme legcons:Item .

F2021L00315:211 a legcons:Item,
        owl:Class,
        dcat:Resource ;
    rdfs:label "Item - I211 9 32  Certain approved containers must be sealed with tamper evident seal"@en-AU ;
    dct:isPartOf F2021L00315:208 ;
    dct:isReferencedBy F2021L00315: ;
    rdfs:comment "9 32  Certain approved containers must be sealed with tamper evident seal - Abrievated Graph Key: I211"@en-AU ;
    skos:definition "9 32  Certain approved containers must be sealed with tamper evident seal"@en-AU ;
    skos:narrower F2021L00315:208 ;
    skos:prefLabel "Item I211"@en-AU ;
    dcat:accessURL <https://www.legislation.gov.au/F2021L00315/2023-08-04/2023-08-04/text/original/epub/OEBPS/document_1/document_1.html#_Toc143854035> ;
    dcat:landingPage "https://www.legislation.gov.au/F2021L00315/2023-08-04/2023-08-04/text/original/epub/OEBPS/document_1/document_1.html#_Toc143854035"^^xsd:anyURI ;
    dcat:theme legcons:Item .

F2021L00315:212 a legcons:Item,
        owl:Class,
        dcat:Resource ;
    rdfs:label "Item - I212 9 33  Container inspection record"@en-AU ;
    dct:isPartOf F2021L00315:208 ;
    dct:isReferencedBy F2021L00315: ;
    rdfs:comment "9 33  Container inspection record - Abrievated Graph Key: I212"@en-AU ;
    skos:definition "9 33  Container inspection record"@en-AU ;
    skos:narrower F2021L00315:208 ;
    skos:prefLabel "Item I212"@en-AU ;
    dcat:accessURL <https://www.legislation.gov.au/F2021L00315/2023-08-04/2023-08-04/text/original/epub/OEBPS/document_1/document_1.html#_Toc143854036> ;
    dcat:landingPage "https://www.legislation.gov.au/F2021L00315/2023-08-04/2023-08-04/text/original/epub/OEBPS/document_1/document_1.html#_Toc143854036"^^xsd:anyURI ;
    dcat:theme legcons:Item .

F2021L00315:213 a legcons:Item,
        owl:Class,
        dcat:Resource ;
    rdfs:label "Item - I213 9 34  Period of effect of container approval"@en-AU ;
    dct:isPartOf F2021L00315:208 ;
    dct:isReferencedBy F2021L00315: ;
    rdfs:comment "9 34  Period of effect of container approval - Abrievated Graph Key: I213"@en-AU ;
    skos:definition "9 34  Period of effect of container approval"@en-AU ;
    skos:narrower F2021L00315:208 ;
    skos:prefLabel "Item I213"@en-AU ;
    dcat:accessURL <https://www.legislation.gov.au/F2021L00315/2023-08-04/2023-08-04/text/original/epub/OEBPS/document_1/document_1.html#_Toc143854037> ;
    dcat:landingPage "https://www.legislation.gov.au/F2021L00315/2023-08-04/2023-08-04/text/original/epub/OEBPS/document_1/document_1.html#_Toc143854037"^^xsd:anyURI ;
    dcat:theme legcons:Item .

F2021L00315:214 a legcons:Item,
        owl:Class,
        dcat:Resource ;
    rdfs:label "Item - I214 9 35  Extension of period of effect of container approval"@en-AU ;
    dct:isPartOf F2021L00315:208 ;
    dct:isReferencedBy F2021L00315: ;
    rdfs:comment "9 35  Extension of period of effect of container approval - Abrievated Graph Key: I214"@en-AU ;
    skos:definition "9 35  Extension of period of effect of container approval"@en-AU ;
    skos:narrower F2021L00315:208 ;
    skos:prefLabel "Item I214"@en-AU ;
    dcat:accessURL <https://www.legislation.gov.au/F2021L00315/2023-08-04/2023-08-04/text/original/epub/OEBPS/document_1/document_1.html#_Toc143854038> ;
    dcat:landingPage "https://www.legislation.gov.au/F2021L00315/2023-08-04/2023-08-04/text/original/epub/OEBPS/document_1/document_1.html#_Toc143854038"^^xsd:anyURI ;
    dcat:theme legcons:Item .

F2021L00315:215 a legcons:Item,
        owl:Class,
        dcat:Resource ;
    rdfs:label "Item - I215 9 36  Revocation of container approval"@en-AU ;
    dct:isPartOf F2021L00315:208 ;
    dct:isReferencedBy F2021L00315: ;
    rdfs:comment "9 36  Revocation of container approval - Abrievated Graph Key: I215"@en-AU ;
    skos:definition "9 36  Revocation of container approval"@en-AU ;
    skos:narrower F2021L00315:208 ;
    skos:prefLabel "Item I215"@en-AU ;
    dcat:accessURL <https://www.legislation.gov.au/F2021L00315/2023-08-04/2023-08-04/text/original/epub/OEBPS/document_1/document_1.html#_Toc143854039> ;
    dcat:landingPage "https://www.legislation.gov.au/F2021L00315/2023-08-04/2023-08-04/text/original/epub/OEBPS/document_1/document_1.html#_Toc143854039"^^xsd:anyURI ;
    dcat:theme legcons:Item .

F2021L00315:217 a legcons:Item,
        owl:Class,
        dcat:Resource ;
    rdfs:label "Item - I217 10 1  Samples taken in exercising monitoring or investigation powers"@en-AU ;
    dct:isPartOf F2021L00315:216 ;
    dct:isReferencedBy F2021L00315: ;
    rdfs:comment "10 1  Samples taken in exercising monitoring or investigation powers - Abrievated Graph Key: I217"@en-AU ;
    skos:definition "10 1  Samples taken in exercising monitoring or investigation powers"@en-AU ;
    skos:narrower F2021L00315:216 ;
    skos:prefLabel "Item I217"@en-AU ;
    dcat:accessURL <https://www.legislation.gov.au/F2021L00315/2023-08-04/2023-08-04/text/original/epub/OEBPS/document_1/document_1.html#_Toc143854041> ;
    dcat:landingPage "https://www.legislation.gov.au/F2021L00315/2023-08-04/2023-08-04/text/original/epub/OEBPS/document_1/document_1.html#_Toc143854041"^^xsd:anyURI ;
    dcat:theme legcons:Item .

F2021L00315:218 a legcons:Item,
        owl:Class,
        dcat:Resource ;
    rdfs:label "Item - I218 10 2  Dealing with things seized in exercising investigation powers"@en-AU ;
    dct:isPartOf F2021L00315:216 ;
    dct:isReferencedBy F2021L00315: ;
    rdfs:comment "10 2  Dealing with things seized in exercising investigation powers - Abrievated Graph Key: I218"@en-AU ;
    skos:definition "10 2  Dealing with things seized in exercising investigation powers"@en-AU ;
    skos:narrower F2021L00315:216 ;
    skos:prefLabel "Item I218"@en-AU ;
    dcat:accessURL <https://www.legislation.gov.au/F2021L00315/2023-08-04/2023-08-04/text/original/epub/OEBPS/document_1/document_1.html#_Toc143854042> ;
    dcat:landingPage "https://www.legislation.gov.au/F2021L00315/2023-08-04/2023-08-04/text/original/epub/OEBPS/document_1/document_1.html#_Toc143854042"^^xsd:anyURI ;
    dcat:theme legcons:Item .

F2021L00315:22 a legcons:Item,
        owl:Class,
        dcat:Resource ;
    rdfs:label "Item - I22 2 7  Conditions of exemptionmatters to which Secretary must have regard"@en-AU ;
    dct:isPartOf F2021L00315:11 ;
    dct:isReferencedBy F2021L00315: ;
    rdfs:comment "2 7  Conditions of exemptionmatters to which Secretary must have regard - Abrievated Graph Key: I22"@en-AU ;
    skos:definition "2 7  Conditions of exemptionmatters to which Secretary must have regard"@en-AU ;
    skos:narrower F2021L00315:11 ;
    skos:prefLabel "Item I22"@en-AU ;
    dcat:accessURL <https://www.legislation.gov.au/F2021L00315/2023-08-04/2023-08-04/text/original/epub/OEBPS/document_1/document_1.html#_Toc143853846> ;
    dcat:landingPage "https://www.legislation.gov.au/F2021L00315/2023-08-04/2023-08-04/text/original/epub/OEBPS/document_1/document_1.html#_Toc143853846"^^xsd:anyURI ;
    dcat:theme legcons:Item .

F2021L00315:221 a legcons:Item,
        owl:Class,
        dcat:Resource ;
    rdfs:label "Item - I221 11 1  Purpose of this Part"@en-AU ;
    dct:isPartOf F2021L00315:220 ;
    dct:isReferencedBy F2021L00315: ;
    rdfs:comment "11 1  Purpose of this Part - Abrievated Graph Key: I221"@en-AU ;
    skos:definition "11 1  Purpose of this Part"@en-AU ;
    skos:narrower F2021L00315:220 ;
    skos:prefLabel "Item I221"@en-AU ;
    dcat:accessURL <https://www.legislation.gov.au/F2021L00315/2023-08-04/2023-08-04/text/original/epub/OEBPS/document_1/document_1.html#_Toc143854045> ;
    dcat:landingPage "https://www.legislation.gov.au/F2021L00315/2023-08-04/2023-08-04/text/original/epub/OEBPS/document_1/document_1.html#_Toc143854045"^^xsd:anyURI ;
    dcat:theme legcons:Item .

F2021L00315:222 a legcons:Item,
        owl:Class,
        dcat:Resource ;
    rdfs:label "Item - I222 11 2  General requirements for records"@en-AU ;
    dct:isPartOf F2021L00315:220 ;
    dct:isReferencedBy F2021L00315: ;
    rdfs:comment "11 2  General requirements for records - Abrievated Graph Key: I222"@en-AU ;
    skos:definition "11 2  General requirements for records"@en-AU ;
    skos:narrower F2021L00315:220 ;
    skos:prefLabel "Item I222"@en-AU ;
    dcat:accessURL <https://www.legislation.gov.au/F2021L00315/2023-08-04/2023-08-04/text/original/epub/OEBPS/document_1/document_1.html#_Toc143854046> ;
    dcat:landingPage "https://www.legislation.gov.au/F2021L00315/2023-08-04/2023-08-04/text/original/epub/OEBPS/document_1/document_1.html#_Toc143854046"^^xsd:anyURI ;
    dcat:theme legcons:Item .

F2021L00315:223 a legcons:Item,
        owl:Class,
        dcat:Resource ;
    rdfs:label "Item - I223 11 3  Government certificates must be retained in secure place"@en-AU ;
    dct:isPartOf F2021L00315:220 ;
    dct:isReferencedBy F2021L00315: ;
    rdfs:comment "11 3  Government certificates must be retained in secure place - Abrievated Graph Key: I223"@en-AU ;
    skos:definition "11 3  Government certificates must be retained in secure place"@en-AU ;
    skos:narrower F2021L00315:220 ;
    skos:prefLabel "Item I223"@en-AU ;
    dcat:accessURL <https://www.legislation.gov.au/F2021L00315/2023-08-04/2023-08-04/text/original/epub/OEBPS/document_1/document_1.html#_Toc143854047> ;
    dcat:landingPage "https://www.legislation.gov.au/F2021L00315/2023-08-04/2023-08-04/text/original/epub/OEBPS/document_1/document_1.html#_Toc143854047"^^xsd:anyURI ;
    dcat:theme legcons:Item .

F2021L00315:224 a legcons:Item,
        owl:Class,
        dcat:Resource ;
    rdfs:label "Item - I224 11 4  Export permits must be retained in secure place"@en-AU ;
    dct:isPartOf F2021L00315:220 ;
    dct:isReferencedBy F2021L00315: ;
    rdfs:comment "11 4  Export permits must be retained in secure place - Abrievated Graph Key: I224"@en-AU ;
    skos:definition "11 4  Export permits must be retained in secure place"@en-AU ;
    skos:narrower F2021L00315:220 ;
    skos:prefLabel "Item I224"@en-AU ;
    dcat:accessURL <https://www.legislation.gov.au/F2021L00315/2023-08-04/2023-08-04/text/original/epub/OEBPS/document_1/document_1.html#_Toc143854048> ;
    dcat:landingPage "https://www.legislation.gov.au/F2021L00315/2023-08-04/2023-08-04/text/original/epub/OEBPS/document_1/document_1.html#_Toc143854048"^^xsd:anyURI ;
    dcat:theme legcons:Item .

F2021L00315:225 a legcons:Item,
        owl:Class,
        dcat:Resource ;
    rdfs:label "Item - I225 11 5  Records to be retained by exporter etc"@en-AU ;
    dct:isPartOf F2021L00315:220 ;
    dct:isReferencedBy F2021L00315: ;
    rdfs:comment "11 5  Records to be retained by exporter etc - Abrievated Graph Key: I225"@en-AU ;
    skos:definition "11 5  Records to be retained by exporter etc"@en-AU ;
    skos:narrower F2021L00315:220 ;
    skos:prefLabel "Item I225"@en-AU ;
    dcat:accessURL <https://www.legislation.gov.au/F2021L00315/2023-08-04/2023-08-04/text/original/epub/OEBPS/document_1/document_1.html#_Toc143854049> ;
    dcat:landingPage "https://www.legislation.gov.au/F2021L00315/2023-08-04/2023-08-04/text/original/epub/OEBPS/document_1/document_1.html#_Toc143854049"^^xsd:anyURI ;
    dcat:theme legcons:Item .

F2021L00315:226 a legcons:Item,
        owl:Class,
        dcat:Resource ;
    rdfs:label "Item - I226 11 6  Records to be retained by manager of accredited property"@en-AU ;
    dct:isPartOf F2021L00315:220 ;
    dct:isReferencedBy F2021L00315: ;
    rdfs:comment "11 6  Records to be retained by manager of accredited property - Abrievated Graph Key: I226"@en-AU ;
    skos:definition "11 6  Records to be retained by manager of accredited property"@en-AU ;
    skos:narrower F2021L00315:220 ;
    skos:prefLabel "Item I226"@en-AU ;
    dcat:accessURL <https://www.legislation.gov.au/F2021L00315/2023-08-04/2023-08-04/text/original/epub/OEBPS/document_1/document_1.html#_Toc143854050> ;
    dcat:landingPage "https://www.legislation.gov.au/F2021L00315/2023-08-04/2023-08-04/text/original/epub/OEBPS/document_1/document_1.html#_Toc143854050"^^xsd:anyURI ;
    dcat:theme legcons:Item .

F2021L00315:227 a legcons:Item,
        owl:Class,
        dcat:Resource ;
    rdfs:label "Item - I227 11 7  Records to be retained by occupier of registered establishment"@en-AU ;
    dct:isPartOf F2021L00315:220 ;
    dct:isReferencedBy F2021L00315: ;
    rdfs:comment "11 7  Records to be retained by occupier of registered establishment - Abrievated Graph Key: I227"@en-AU ;
    skos:definition "11 7  Records to be retained by occupier of registered establishment"@en-AU ;
    skos:narrower F2021L00315:220 ;
    skos:prefLabel "Item I227"@en-AU ;
    dcat:accessURL <https://www.legislation.gov.au/F2021L00315/2023-08-04/2023-08-04/text/original/epub/OEBPS/document_1/document_1.html#_Toc143854051> ;
    dcat:landingPage "https://www.legislation.gov.au/F2021L00315/2023-08-04/2023-08-04/text/original/epub/OEBPS/document_1/document_1.html#_Toc143854051"^^xsd:anyURI ;
    dcat:theme legcons:Item .

F2021L00315:228 a legcons:Item,
        owl:Class,
        dcat:Resource ;
    rdfs:label "Item - I228 11 8  Records relating to official marks"@en-AU ;
    dct:isPartOf F2021L00315:220 ;
    dct:isReferencedBy F2021L00315: ;
    rdfs:comment "11 8  Records relating to official marks - Abrievated Graph Key: I228"@en-AU ;
    skos:definition "11 8  Records relating to official marks"@en-AU ;
    skos:narrower F2021L00315:220 ;
    skos:prefLabel "Item I228"@en-AU ;
    dcat:accessURL <https://www.legislation.gov.au/F2021L00315/2023-08-04/2023-08-04/text/original/epub/OEBPS/document_1/document_1.html#_Toc143854052> ;
    dcat:landingPage "https://www.legislation.gov.au/F2021L00315/2023-08-04/2023-08-04/text/original/epub/OEBPS/document_1/document_1.html#_Toc143854052"^^xsd:anyURI ;
    dcat:theme legcons:Item .

F2021L00315:229 a legcons:Item,
        owl:Class,
        dcat:Resource ;
    rdfs:label "Item - I229 11 9  Records relating to official marking devices"@en-AU ;
    dct:isPartOf F2021L00315:220 ;
    dct:isReferencedBy F2021L00315: ;
    rdfs:comment "11 9  Records relating to official marking devices - Abrievated Graph Key: I229"@en-AU ;
    skos:definition "11 9  Records relating to official marking devices"@en-AU ;
    skos:narrower F2021L00315:220 ;
    skos:prefLabel "Item I229"@en-AU ;
    dcat:accessURL <https://www.legislation.gov.au/F2021L00315/2023-08-04/2023-08-04/text/original/epub/OEBPS/document_1/document_1.html#_Toc143854053> ;
    dcat:landingPage "https://www.legislation.gov.au/F2021L00315/2023-08-04/2023-08-04/text/original/epub/OEBPS/document_1/document_1.html#_Toc143854053"^^xsd:anyURI ;
    dcat:theme legcons:Item .

F2021L00315:23 a legcons:Item,
        owl:Class,
        dcat:Resource ;
    rdfs:label "Item - I23 2 8  Period of effect of exemption"@en-AU ;
    dct:isPartOf F2021L00315:11 ;
    dct:isReferencedBy F2021L00315: ;
    rdfs:comment "2 8  Period of effect of exemption - Abrievated Graph Key: I23"@en-AU ;
    skos:definition "2 8  Period of effect of exemption"@en-AU ;
    skos:narrower F2021L00315:11 ;
    skos:prefLabel "Item I23"@en-AU ;
    dcat:accessURL <https://www.legislation.gov.au/F2021L00315/2023-08-04/2023-08-04/text/original/epub/OEBPS/document_1/document_1.html#_Toc143853847> ;
    dcat:landingPage "https://www.legislation.gov.au/F2021L00315/2023-08-04/2023-08-04/text/original/epub/OEBPS/document_1/document_1.html#_Toc143853847"^^xsd:anyURI ;
    dcat:theme legcons:Item .

F2021L00315:230 a legcons:Item,
        owl:Class,
        dcat:Resource ;
    rdfs:label "Item - I230 11 10  Records to be retained by authorised officers"@en-AU ;
    dct:isPartOf F2021L00315:220 ;
    dct:isReferencedBy F2021L00315: ;
    rdfs:comment "11 10  Records to be retained by authorised officers - Abrievated Graph Key: I230"@en-AU ;
    skos:definition "11 10  Records to be retained by authorised officers"@en-AU ;
    skos:narrower F2021L00315:220 ;
    skos:prefLabel "Item I230"@en-AU ;
    dcat:accessURL <https://www.legislation.gov.au/F2021L00315/2023-08-04/2023-08-04/text/original/epub/OEBPS/document_1/document_1.html#_Toc143854054> ;
    dcat:landingPage "https://www.legislation.gov.au/F2021L00315/2023-08-04/2023-08-04/text/original/epub/OEBPS/document_1/document_1.html#_Toc143854054"^^xsd:anyURI ;
    dcat:theme legcons:Item .

F2021L00315:231 a legcons:Item,
        owl:Class,
        dcat:Resource ;
    rdfs:label "Item - I231 11 11  Records must not be altered or defaced during retention period"@en-AU ;
    dct:isPartOf F2021L00315:220 ;
    dct:isReferencedBy F2021L00315: ;
    rdfs:comment "11 11  Records must not be altered or defaced during retention period - Abrievated Graph Key: I231"@en-AU ;
    skos:definition "11 11  Records must not be altered or defaced during retention period"@en-AU ;
    skos:narrower F2021L00315:220 ;
    skos:prefLabel "Item I231"@en-AU ;
    dcat:accessURL <https://www.legislation.gov.au/F2021L00315/2023-08-04/2023-08-04/text/original/epub/OEBPS/document_1/document_1.html#_Toc143854055> ;
    dcat:landingPage "https://www.legislation.gov.au/F2021L00315/2023-08-04/2023-08-04/text/original/epub/OEBPS/document_1/document_1.html#_Toc143854055"^^xsd:anyURI ;
    dcat:theme legcons:Item .

F2021L00315:233 a legcons:Item,
        owl:Class,
        dcat:Resource ;
    rdfs:label "Item - I233 11 12  Storage of samples"@en-AU ;
    dct:isPartOf F2021L00315:232 ;
    dct:isReferencedBy F2021L00315: ;
    rdfs:comment "11 12  Storage of samples - Abrievated Graph Key: I233"@en-AU ;
    skos:definition "11 12  Storage of samples"@en-AU ;
    skos:narrower F2021L00315:232 ;
    skos:prefLabel "Item I233"@en-AU ;
    dcat:accessURL <https://www.legislation.gov.au/F2021L00315/2023-08-04/2023-08-04/text/original/epub/OEBPS/document_1/document_1.html#_Toc143854057> ;
    dcat:landingPage "https://www.legislation.gov.au/F2021L00315/2023-08-04/2023-08-04/text/original/epub/OEBPS/document_1/document_1.html#_Toc143854057"^^xsd:anyURI ;
    dcat:theme legcons:Item .

F2021L00315:235 a legcons:Item,
        owl:Class,
        dcat:Resource ;
    rdfs:label "Item - I235 11 13  Division of compensation between owners"@en-AU ;
    dct:isPartOf F2021L00315:234 ;
    dct:isReferencedBy F2021L00315: ;
    rdfs:comment "11 13  Division of compensation between owners - Abrievated Graph Key: I235"@en-AU ;
    skos:definition "11 13  Division of compensation between owners"@en-AU ;
    skos:narrower F2021L00315:234 ;
    skos:prefLabel "Item I235"@en-AU ;
    dcat:accessURL <https://www.legislation.gov.au/F2021L00315/2023-08-04/2023-08-04/text/original/epub/OEBPS/document_1/document_1.html#_Toc143854059> ;
    dcat:landingPage "https://www.legislation.gov.au/F2021L00315/2023-08-04/2023-08-04/text/original/epub/OEBPS/document_1/document_1.html#_Toc143854059"^^xsd:anyURI ;
    dcat:theme legcons:Item .

F2021L00315:236 a legcons:Item,
        owl:Class,
        dcat:Resource ;
    rdfs:label "Item - I236 11 14  Amount of compensation"@en-AU ;
    dct:isPartOf F2021L00315:234 ;
    dct:isReferencedBy F2021L00315: ;
    rdfs:comment "11 14  Amount of compensation - Abrievated Graph Key: I236"@en-AU ;
    skos:definition "11 14  Amount of compensation"@en-AU ;
    skos:narrower F2021L00315:234 ;
    skos:prefLabel "Item I236"@en-AU ;
    dcat:accessURL <https://www.legislation.gov.au/F2021L00315/2023-08-04/2023-08-04/text/original/epub/OEBPS/document_1/document_1.html#_Toc143854060> ;
    dcat:landingPage "https://www.legislation.gov.au/F2021L00315/2023-08-04/2023-08-04/text/original/epub/OEBPS/document_1/document_1.html#_Toc143854060"^^xsd:anyURI ;
    dcat:theme legcons:Item .

F2021L00315:238 a legcons:Item,
        owl:Class,
        dcat:Resource ;
    rdfs:label "Item - I238 11 15  Circumstances in which relevant Commonwealth liability of a person is taken to have been paid"@en-AU ;
    dct:isPartOf F2021L00315:237 ;
    dct:isReferencedBy F2021L00315: ;
    rdfs:comment "11 15  Circumstances in which relevant Commonwealth liability of a person is taken to have been paid - Abrievated Graph Key: I238"@en-AU ;
    skos:definition "11 15  Circumstances in which relevant Commonwealth liability of a person is taken to have been paid"@en-AU ;
    skos:narrower F2021L00315:237 ;
    skos:prefLabel "Item I238"@en-AU ;
    dcat:accessURL <https://www.legislation.gov.au/F2021L00315/2023-08-04/2023-08-04/text/original/epub/OEBPS/document_1/document_1.html#_Toc143854062> ;
    dcat:landingPage "https://www.legislation.gov.au/F2021L00315/2023-08-04/2023-08-04/text/original/epub/OEBPS/document_1/document_1.html#_Toc143854062"^^xsd:anyURI ;
    dcat:theme legcons:Item .

F2021L00315:24 a legcons:Item,
        owl:Class,
        dcat:Resource ;
    rdfs:label "Item - I24 2 9  Variation of conditions of exemptionmatters to which Secretary must have regard"@en-AU ;
    dct:isPartOf F2021L00315:11 ;
    dct:isReferencedBy F2021L00315: ;
    rdfs:comment "2 9  Variation of conditions of exemptionmatters to which Secretary must have regard - Abrievated Graph Key: I24"@en-AU ;
    skos:definition "2 9  Variation of conditions of exemptionmatters to which Secretary must have regard"@en-AU ;
    skos:narrower F2021L00315:11 ;
    skos:prefLabel "Item I24"@en-AU ;
    dcat:accessURL <https://www.legislation.gov.au/F2021L00315/2023-08-04/2023-08-04/text/original/epub/OEBPS/document_1/document_1.html#_Toc143853848> ;
    dcat:landingPage "https://www.legislation.gov.au/F2021L00315/2023-08-04/2023-08-04/text/original/epub/OEBPS/document_1/document_1.html#_Toc143853848"^^xsd:anyURI ;
    dcat:theme legcons:Item .

F2021L00315:240 a legcons:Item,
        owl:Class,
        dcat:Resource ;
    rdfs:label "Item - I240 11 16  Accredited marine surveyors and marine surveyors certificates"@en-AU ;
    dct:isPartOf F2021L00315:239 ;
    dct:isReferencedBy F2021L00315: ;
    rdfs:comment "11 16  Accredited marine surveyors and marine surveyors certificates - Abrievated Graph Key: I240"@en-AU ;
    skos:definition "11 16  Accredited marine surveyors and marine surveyors certificates"@en-AU ;
    skos:narrower F2021L00315:239 ;
    skos:prefLabel "Item I240"@en-AU ;
    dcat:accessURL <https://www.legislation.gov.au/F2021L00315/2023-08-04/2023-08-04/text/original/epub/OEBPS/document_1/document_1.html#_Toc143854064> ;
    dcat:landingPage "https://www.legislation.gov.au/F2021L00315/2023-08-04/2023-08-04/text/original/epub/OEBPS/document_1/document_1.html#_Toc143854064"^^xsd:anyURI ;
    dcat:theme legcons:Item .

F2021L00315:243 a legcons:Item,
        owl:Class,
        dcat:Resource ;
    rdfs:label "Item - I243 12 1  Definitions"@en-AU ;
    dct:isPartOf F2021L00315:242 ;
    dct:isReferencedBy F2021L00315: ;
    rdfs:comment "12 1  Definitions - Abrievated Graph Key: I243"@en-AU ;
    skos:definition "12 1  Definitions"@en-AU ;
    skos:narrower F2021L00315:242 ;
    skos:prefLabel "Item I243"@en-AU ;
    dcat:accessURL <https://www.legislation.gov.au/F2021L00315/2023-08-04/2023-08-04/text/original/epub/OEBPS/document_1/document_1.html#_Toc143854067> ;
    dcat:landingPage "https://www.legislation.gov.au/F2021L00315/2023-08-04/2023-08-04/text/original/epub/OEBPS/document_1/document_1.html#_Toc143854067"^^xsd:anyURI ;
    dcat:theme legcons:Item .

F2021L00315:245 a legcons:Item,
        owl:Class,
        dcat:Resource ;
    rdfs:label "Item - I245 12 2  Application for determination that establishment is a small horticultural products registered establishment for a financial year"@en-AU ;
    dct:isPartOf F2021L00315:244 ;
    dct:isReferencedBy F2021L00315: ;
    rdfs:comment "12 2  Application for determination that establishment is a small horticultural products registered establishment for a financial year - Abrievated Graph Key: I245"@en-AU ;
    skos:definition "12 2  Application for determination that establishment is a small horticultural products registered establishment for a financial year"@en-AU ;
    skos:narrower F2021L00315:244 ;
    skos:prefLabel "Item I245"@en-AU ;
    dcat:accessURL <https://www.legislation.gov.au/F2021L00315/2023-08-04/2023-08-04/text/original/epub/OEBPS/document_1/document_1.html#_Toc143854069> ;
    dcat:landingPage "https://www.legislation.gov.au/F2021L00315/2023-08-04/2023-08-04/text/original/epub/OEBPS/document_1/document_1.html#_Toc143854069"^^xsd:anyURI ;
    dcat:theme legcons:Item .

F2021L00315:246 a legcons:Item,
        owl:Class,
        dcat:Resource ;
    rdfs:label "Item - I246 12 3  Determination in force that establishment is a small horticultural products registered establishment for financial year ending on 30 June 2021"@en-AU ;
    dct:isPartOf F2021L00315:244 ;
    dct:isReferencedBy F2021L00315: ;
    rdfs:comment "12 3  Determination in force that establishment is a small horticultural products registered establishment for financial year ending on 30 June 2021 - Abrievated Graph Key: I246"@en-AU ;
    skos:definition "12 3  Determination in force that establishment is a small horticultural products registered establishment for financial year ending on 30 June 2021"@en-AU ;
    skos:narrower F2021L00315:244 ;
    skos:prefLabel "Item I246"@en-AU ;
    dcat:accessURL <https://www.legislation.gov.au/F2021L00315/2023-08-04/2023-08-04/text/original/epub/OEBPS/document_1/document_1.html#_Toc143854070> ;
    dcat:landingPage "https://www.legislation.gov.au/F2021L00315/2023-08-04/2023-08-04/text/original/epub/OEBPS/document_1/document_1.html#_Toc143854070"^^xsd:anyURI ;
    dcat:theme legcons:Item .

F2021L00315:249 a legcons:Item,
        owl:Class,
        dcat:Resource ;
    rdfs:label "Item - I249 12 4  Person approved before commencement time to manufacture an official mark"@en-AU ;
    dct:isPartOf F2021L00315:248 ;
    dct:isReferencedBy F2021L00315: ;
    rdfs:comment "12 4  Person approved before commencement time to manufacture an official mark - Abrievated Graph Key: I249"@en-AU ;
    skos:definition "12 4  Person approved before commencement time to manufacture an official mark"@en-AU ;
    skos:narrower F2021L00315:248 ;
    skos:prefLabel "Item I249"@en-AU ;
    dcat:accessURL <https://www.legislation.gov.au/F2021L00315/2023-08-04/2023-08-04/text/original/epub/OEBPS/document_1/document_1.html#_Toc143854073> ;
    dcat:landingPage "https://www.legislation.gov.au/F2021L00315/2023-08-04/2023-08-04/text/original/epub/OEBPS/document_1/document_1.html#_Toc143854073"^^xsd:anyURI ;
    dcat:theme legcons:Item .

F2021L00315:25 a legcons:Part,
        owl:Class,
        dcat:Resource ;
    rdfs:label "Part - P25 Part 3 Government certificates"@en-AU ;
    dct:isPartOf F2021L00315:11 ;
    dct:isReferencedBy F2021L00315: ;
    rdfs:comment "Part 3 Government certificates - Abrievated Graph Key: P25"@en-AU ;
    skos:definition "Part 3 Government certificates"@en-AU ;
    skos:narrower F2021L00315:11 ;
    skos:prefLabel "Part P25"@en-AU ;
    dcat:accessURL <https://www.legislation.gov.au/F2021L00315/2023-08-04/2023-08-04/text/original/epub/OEBPS/document_1/document_1.html#_Toc143853849> ;
    dcat:landingPage "https://www.legislation.gov.au/F2021L00315/2023-08-04/2023-08-04/text/original/epub/OEBPS/document_1/document_1.html#_Toc143853849"^^xsd:anyURI ;
    dcat:theme legcons:Part .

F2021L00315:250 a legcons:Item,
        owl:Class,
        dcat:Resource ;
    rdfs:label "Item - I250 12 5  Persons permitted before commencement time to possess an official mark"@en-AU ;
    dct:isPartOf F2021L00315:248 ;
    dct:isReferencedBy F2021L00315: ;
    rdfs:comment "12 5  Persons permitted before commencement time to possess an official mark - Abrievated Graph Key: I250"@en-AU ;
    skos:definition "12 5  Persons permitted before commencement time to possess an official mark"@en-AU ;
    skos:narrower F2021L00315:248 ;
    skos:prefLabel "Item I250"@en-AU ;
    dcat:accessURL <https://www.legislation.gov.au/F2021L00315/2023-08-04/2023-08-04/text/original/epub/OEBPS/document_1/document_1.html#_Toc143854074> ;
    dcat:landingPage "https://www.legislation.gov.au/F2021L00315/2023-08-04/2023-08-04/text/original/epub/OEBPS/document_1/document_1.html#_Toc143854074"^^xsd:anyURI ;
    dcat:theme legcons:Item .

F2021L00315:251 a legcons:Item,
        owl:Class,
        dcat:Resource ;
    rdfs:label "Item - I251 12 6  Persons permitted before commencement time to apply an official mark"@en-AU ;
    dct:isPartOf F2021L00315:248 ;
    dct:isReferencedBy F2021L00315: ;
    rdfs:comment "12 6  Persons permitted before commencement time to apply an official mark - Abrievated Graph Key: I251"@en-AU ;
    skos:definition "12 6  Persons permitted before commencement time to apply an official mark"@en-AU ;
    skos:narrower F2021L00315:248 ;
    skos:prefLabel "Item I251"@en-AU ;
    dcat:accessURL <https://www.legislation.gov.au/F2021L00315/2023-08-04/2023-08-04/text/original/epub/OEBPS/document_1/document_1.html#_Toc143854075> ;
    dcat:landingPage "https://www.legislation.gov.au/F2021L00315/2023-08-04/2023-08-04/text/original/epub/OEBPS/document_1/document_1.html#_Toc143854075"^^xsd:anyURI ;
    dcat:theme legcons:Item .

F2021L00315:253 a legcons:Item,
        owl:Class,
        dcat:Resource ;
    rdfs:label "Item - I253 12 7  Person approved before commencement time to manufacture an official marking device"@en-AU ;
    dct:isPartOf F2021L00315:252 ;
    dct:isReferencedBy F2021L00315: ;
    rdfs:comment "12 7  Person approved before commencement time to manufacture an official marking device - Abrievated Graph Key: I253"@en-AU ;
    skos:definition "12 7  Person approved before commencement time to manufacture an official marking device"@en-AU ;
    skos:narrower F2021L00315:252 ;
    skos:prefLabel "Item I253"@en-AU ;
    dcat:accessURL <https://www.legislation.gov.au/F2021L00315/2023-08-04/2023-08-04/text/original/epub/OEBPS/document_1/document_1.html#_Toc143854077> ;
    dcat:landingPage "https://www.legislation.gov.au/F2021L00315/2023-08-04/2023-08-04/text/original/epub/OEBPS/document_1/document_1.html#_Toc143854077"^^xsd:anyURI ;
    dcat:theme legcons:Item .

F2021L00315:254 a legcons:Item,
        owl:Class,
        dcat:Resource ;
    rdfs:label "Item - I254 12 8  Person approved before commencement time to possess an official marking device"@en-AU ;
    dct:isPartOf F2021L00315:252 ;
    dct:isReferencedBy F2021L00315: ;
    rdfs:comment "12 8  Person approved before commencement time to possess an official marking device - Abrievated Graph Key: I254"@en-AU ;
    skos:definition "12 8  Person approved before commencement time to possess an official marking device"@en-AU ;
    skos:narrower F2021L00315:252 ;
    skos:prefLabel "Item I254"@en-AU ;
    dcat:accessURL <https://www.legislation.gov.au/F2021L00315/2023-08-04/2023-08-04/text/original/epub/OEBPS/document_1/document_1.html#_Toc143854078> ;
    dcat:landingPage "https://www.legislation.gov.au/F2021L00315/2023-08-04/2023-08-04/text/original/epub/OEBPS/document_1/document_1.html#_Toc143854078"^^xsd:anyURI ;
    dcat:theme legcons:Item .

F2021L00315:257 a legcons:Item,
        owl:Class,
        dcat:Resource ;
    rdfs:label "Item - I257 12 9  Declaration by authorised officer before commencement time that prescribed goods are passed as export compliant"@en-AU ;
    dct:isPartOf F2021L00315:256 ;
    dct:isReferencedBy F2021L00315: ;
    rdfs:comment "12 9  Declaration by authorised officer before commencement time that prescribed goods are passed as export compliant - Abrievated Graph Key: I257"@en-AU ;
    skos:definition "12 9  Declaration by authorised officer before commencement time that prescribed goods are passed as export compliant"@en-AU ;
    skos:narrower F2021L00315:256 ;
    skos:prefLabel "Item I257"@en-AU ;
    dcat:accessURL <https://www.legislation.gov.au/F2021L00315/2023-08-04/2023-08-04/text/original/epub/OEBPS/document_1/document_1.html#_Toc143854081> ;
    dcat:landingPage "https://www.legislation.gov.au/F2021L00315/2023-08-04/2023-08-04/text/original/epub/OEBPS/document_1/document_1.html#_Toc143854081"^^xsd:anyURI ;
    dcat:theme legcons:Item .

F2021L00315:259 a legcons:Item,
        owl:Class,
        dcat:Resource ;
    rdfs:label "Item - I259 12 10  Marine surveyors certificate issued in relation to bulk vessel before commencement time"@en-AU ;
    dct:isPartOf F2021L00315:258 ;
    dct:isReferencedBy F2021L00315: ;
    rdfs:comment "12 10  Marine surveyors certificate issued in relation to bulk vessel before commencement time - Abrievated Graph Key: I259"@en-AU ;
    skos:definition "12 10  Marine surveyors certificate issued in relation to bulk vessel before commencement time"@en-AU ;
    skos:narrower F2021L00315:258 ;
    skos:prefLabel "Item I259"@en-AU ;
    dcat:accessURL <https://www.legislation.gov.au/F2021L00315/2023-08-04/2023-08-04/text/original/epub/OEBPS/document_1/document_1.html#_Toc143854083> ;
    dcat:landingPage "https://www.legislation.gov.au/F2021L00315/2023-08-04/2023-08-04/text/original/epub/OEBPS/document_1/document_1.html#_Toc143854083"^^xsd:anyURI ;
    dcat:theme legcons:Item .

F2021L00315:260 a legcons:Item,
        owl:Class,
        dcat:Resource ;
    rdfs:label "Item - I260 12 11  Bulk vessel approval in force before commencement time"@en-AU ;
    dct:isPartOf F2021L00315:258 ;
    dct:isReferencedBy F2021L00315: ;
    rdfs:comment "12 11  Bulk vessel approval in force before commencement time - Abrievated Graph Key: I260"@en-AU ;
    skos:definition "12 11  Bulk vessel approval in force before commencement time"@en-AU ;
    skos:narrower F2021L00315:258 ;
    skos:prefLabel "Item I260"@en-AU ;
    dcat:accessURL <https://www.legislation.gov.au/F2021L00315/2023-08-04/2023-08-04/text/original/epub/OEBPS/document_1/document_1.html#_Toc143854084> ;
    dcat:landingPage "https://www.legislation.gov.au/F2021L00315/2023-08-04/2023-08-04/text/original/epub/OEBPS/document_1/document_1.html#_Toc143854084"^^xsd:anyURI ;
    dcat:theme legcons:Item .

F2021L00315:261 a legcons:Item,
        owl:Class,
        dcat:Resource ;
    rdfs:label "Item - I261 12 12  Bulk vessel approval suspended before commencement time"@en-AU ;
    dct:isPartOf F2021L00315:258 ;
    dct:isReferencedBy F2021L00315: ;
    rdfs:comment "12 12  Bulk vessel approval suspended before commencement time - Abrievated Graph Key: I261"@en-AU ;
    skos:definition "12 12  Bulk vessel approval suspended before commencement time"@en-AU ;
    skos:narrower F2021L00315:258 ;
    skos:prefLabel "Item I261"@en-AU ;
    dcat:accessURL <https://www.legislation.gov.au/F2021L00315/2023-08-04/2023-08-04/text/original/epub/OEBPS/document_1/document_1.html#_Toc143854085> ;
    dcat:landingPage "https://www.legislation.gov.au/F2021L00315/2023-08-04/2023-08-04/text/original/epub/OEBPS/document_1/document_1.html#_Toc143854085"^^xsd:anyURI ;
    dcat:theme legcons:Item .

F2021L00315:263 a legcons:Item,
        owl:Class,
        dcat:Resource ;
    rdfs:label "Item - I263 12 13  Container approval in force before commencement time"@en-AU ;
    dct:isPartOf F2021L00315:262 ;
    dct:isReferencedBy F2021L00315: ;
    rdfs:comment "12 13  Container approval in force before commencement time - Abrievated Graph Key: I263"@en-AU ;
    skos:definition "12 13  Container approval in force before commencement time"@en-AU ;
    skos:narrower F2021L00315:262 ;
    skos:prefLabel "Item I263"@en-AU ;
    dcat:accessURL <https://www.legislation.gov.au/F2021L00315/2023-08-04/2023-08-04/text/original/epub/OEBPS/document_1/document_1.html#_Toc143854087> ;
    dcat:landingPage "https://www.legislation.gov.au/F2021L00315/2023-08-04/2023-08-04/text/original/epub/OEBPS/document_1/document_1.html#_Toc143854087"^^xsd:anyURI ;
    dcat:theme legcons:Item .

F2021L00315:265 a legcons:Item,
        owl:Class,
        dcat:Resource ;
    rdfs:label "Item - I265 Endnote 1 About the endnotes"@en-AU ;
    dct:isPartOf F2021L00315:264 ;
    dct:isReferencedBy F2021L00315: ;
    rdfs:comment "Endnote 1 About the endnotes - Abrievated Graph Key: I265"@en-AU ;
    skos:definition "Endnote 1 About the endnotes"@en-AU ;
    skos:narrower F2021L00315:264 ;
    skos:prefLabel "Item I265"@en-AU ;
    dcat:accessURL <https://www.legislation.gov.au/F2021L00315/2023-08-04/2023-08-04/text/original/epub/OEBPS/document_1/document_1.html#_Toc143854089> ;
    dcat:landingPage "https://www.legislation.gov.au/F2021L00315/2023-08-04/2023-08-04/text/original/epub/OEBPS/document_1/document_1.html#_Toc143854089"^^xsd:anyURI ;
    dcat:theme legcons:Item .

F2021L00315:266 a legcons:Item,
        owl:Class,
        dcat:Resource ;
    rdfs:label "Item - I266 Endnote 2 Abbreviation key"@en-AU ;
    dct:isPartOf F2021L00315:264 ;
    dct:isReferencedBy F2021L00315: ;
    rdfs:comment "Endnote 2 Abbreviation key - Abrievated Graph Key: I266"@en-AU ;
    skos:definition "Endnote 2 Abbreviation key"@en-AU ;
    skos:narrower F2021L00315:264 ;
    skos:prefLabel "Item I266"@en-AU ;
    dcat:accessURL <https://www.legislation.gov.au/F2021L00315/2023-08-04/2023-08-04/text/original/epub/OEBPS/document_1/document_1.html#_Toc143854090> ;
    dcat:landingPage "https://www.legislation.gov.au/F2021L00315/2023-08-04/2023-08-04/text/original/epub/OEBPS/document_1/document_1.html#_Toc143854090"^^xsd:anyURI ;
    dcat:theme legcons:Item .

F2021L00315:267 a legcons:Item,
        owl:Class,
        dcat:Resource ;
    rdfs:label "Item - I267 Endnote 3 Legislation history"@en-AU ;
    dct:isPartOf F2021L00315:264 ;
    dct:isReferencedBy F2021L00315: ;
    rdfs:comment "Endnote 3 Legislation history - Abrievated Graph Key: I267"@en-AU ;
    skos:definition "Endnote 3 Legislation history"@en-AU ;
    skos:narrower F2021L00315:264 ;
    skos:prefLabel "Item I267"@en-AU ;
    dcat:accessURL <https://www.legislation.gov.au/F2021L00315/2023-08-04/2023-08-04/text/original/epub/OEBPS/document_1/document_1.html#_Toc143854091> ;
    dcat:landingPage "https://www.legislation.gov.au/F2021L00315/2023-08-04/2023-08-04/text/original/epub/OEBPS/document_1/document_1.html#_Toc143854091"^^xsd:anyURI ;
    dcat:theme legcons:Item .

F2021L00315:268 a legcons:Item,
        owl:Class,
        dcat:Resource ;
    rdfs:label "Item - I268 Endnote 4 Amendment history"@en-AU ;
    dct:isPartOf F2021L00315:264 ;
    dct:isReferencedBy F2021L00315: ;
    rdfs:comment "Endnote 4 Amendment history - Abrievated Graph Key: I268"@en-AU ;
    skos:definition "Endnote 4 Amendment history"@en-AU ;
    skos:narrower F2021L00315:264 ;
    skos:prefLabel "Item I268"@en-AU ;
    dcat:accessURL <https://www.legislation.gov.au/F2021L00315/2023-08-04/2023-08-04/text/original/epub/OEBPS/document_1/document_1.html#_Toc143854092> ;
    dcat:landingPage "https://www.legislation.gov.au/F2021L00315/2023-08-04/2023-08-04/text/original/epub/OEBPS/document_1/document_1.html#_Toc143854092"^^xsd:anyURI ;
    dcat:theme legcons:Item .

F2021L00315:27 a legcons:Item,
        owl:Class,
        dcat:Resource ;
    rdfs:label "Item - I27 2 10  Government certificate may be issued in relation to prescribed plants or plant products"@en-AU ;
    dct:isPartOf F2021L00315:26 ;
    dct:isReferencedBy F2021L00315: ;
    rdfs:comment "2 10  Government certificate may be issued in relation to prescribed plants or plant products - Abrievated Graph Key: I27"@en-AU ;
    skos:definition "2 10  Government certificate may be issued in relation to prescribed plants or plant products"@en-AU ;
    skos:narrower F2021L00315:26 ;
    skos:prefLabel "Item I27"@en-AU ;
    dcat:accessURL <https://www.legislation.gov.au/F2021L00315/2023-08-04/2023-08-04/text/original/epub/OEBPS/document_1/document_1.html#_Toc143853851> ;
    dcat:landingPage "https://www.legislation.gov.au/F2021L00315/2023-08-04/2023-08-04/text/original/epub/OEBPS/document_1/document_1.html#_Toc143853851"^^xsd:anyURI ;
    dcat:theme legcons:Item .

F2021L00315:28 a legcons:Item,
        owl:Class,
        dcat:Resource ;
    rdfs:label "Item - I28 2 11  Phytosanitary certificate or phytosanitary certificate for re export may be issued in relation to non prescribed plants or plant products"@en-AU ;
    dct:isPartOf F2021L00315:26 ;
    dct:isReferencedBy F2021L00315: ;
    rdfs:comment "2 11  Phytosanitary certificate or phytosanitary certificate for re export may be issued in relation to non prescribed plants or plant products - Abrievated Graph Key: I28"@en-AU ;
    skos:definition "2 11  Phytosanitary certificate or phytosanitary certificate for re export may be issued in relation to non prescribed plants or plant products"@en-AU ;
    skos:narrower F2021L00315:26 ;
    skos:prefLabel "Item I28"@en-AU ;
    dcat:accessURL <https://www.legislation.gov.au/F2021L00315/2023-08-04/2023-08-04/text/original/epub/OEBPS/document_1/document_1.html#_Toc143853852> ;
    dcat:landingPage "https://www.legislation.gov.au/F2021L00315/2023-08-04/2023-08-04/text/original/epub/OEBPS/document_1/document_1.html#_Toc143853852"^^xsd:anyURI ;
    dcat:theme legcons:Item .

F2021L00315:3 a legcons:Item,
        owl:Class,
        dcat:Resource ;
    rdfs:label "Item - I3 1 1  Name"@en-AU ;
    dct:isPartOf F2021L00315:1 ;
    dct:isReferencedBy F2021L00315: ;
    rdfs:comment "1 1  Name - Abrievated Graph Key: I3"@en-AU ;
    skos:definition "1 1  Name"@en-AU ;
    skos:narrower F2021L00315:1 ;
    skos:prefLabel "Item I3"@en-AU ;
    dcat:accessURL <https://www.legislation.gov.au/F2021L00315/2023-08-04/2023-08-04/text/original/epub/OEBPS/document_1/document_1.html#_Toc143853827> ;
    dcat:landingPage "https://www.legislation.gov.au/F2021L00315/2023-08-04/2023-08-04/text/original/epub/OEBPS/document_1/document_1.html#_Toc143853827"^^xsd:anyURI ;
    dcat:theme legcons:Item .

F2021L00315:30 a legcons:Item,
        owl:Class,
        dcat:Resource ;
    rdfs:label "Item - I30 2 12  When phytosanitary certificate or phytosanitary certificate for re export in relation to prescribed plants or plant products may be issued"@en-AU ;
    dct:isPartOf F2021L00315:29 ;
    dct:isReferencedBy F2021L00315: ;
    rdfs:comment "2 12  When phytosanitary certificate or phytosanitary certificate for re export in relation to prescribed plants or plant products may be issued - Abrievated Graph Key: I30"@en-AU ;
    skos:definition "2 12  When phytosanitary certificate or phytosanitary certificate for re export in relation to prescribed plants or plant products may be issued"@en-AU ;
    skos:narrower F2021L00315:29 ;
    skos:prefLabel "Item I30"@en-AU ;
    dcat:accessURL <https://www.legislation.gov.au/F2021L00315/2023-08-04/2023-08-04/text/original/epub/OEBPS/document_1/document_1.html#_Toc143853854> ;
    dcat:landingPage "https://www.legislation.gov.au/F2021L00315/2023-08-04/2023-08-04/text/original/epub/OEBPS/document_1/document_1.html#_Toc143853854"^^xsd:anyURI ;
    dcat:theme legcons:Item .

F2021L00315:31 a legcons:Item,
        owl:Class,
        dcat:Resource ;
    rdfs:label "Item - I31 2 13  When phytosanitary certificate or phytosanitary certificate for re export in relation to non prescribed plants or plant products ceases to be in force"@en-AU ;
    dct:isPartOf F2021L00315:29 ;
    dct:isReferencedBy F2021L00315: ;
    rdfs:comment "2 13  When phytosanitary certificate or phytosanitary certificate for re export in relation to non prescribed plants or plant products ceases to be in force - Abrievated Graph Key: I31"@en-AU ;
    skos:definition "2 13  When phytosanitary certificate or phytosanitary certificate for re export in relation to non prescribed plants or plant products ceases to be in force"@en-AU ;
    skos:narrower F2021L00315:29 ;
    skos:prefLabel "Item I31"@en-AU ;
    dcat:accessURL <https://www.legislation.gov.au/F2021L00315/2023-08-04/2023-08-04/text/original/epub/OEBPS/document_1/document_1.html#_Toc143853855> ;
    dcat:landingPage "https://www.legislation.gov.au/F2021L00315/2023-08-04/2023-08-04/text/original/epub/OEBPS/document_1/document_1.html#_Toc143853855"^^xsd:anyURI ;
    dcat:theme legcons:Item .

F2021L00315:33 a legcons:Item,
        owl:Class,
        dcat:Resource ;
    rdfs:label "Item - I33 2 14  Changes that require applicant to give additional or corrected information to issuing body"@en-AU ;
    dct:isPartOf F2021L00315:32 ;
    dct:isReferencedBy F2021L00315: ;
    rdfs:comment "2 14  Changes that require applicant to give additional or corrected information to issuing body - Abrievated Graph Key: I33"@en-AU ;
    skos:definition "2 14  Changes that require applicant to give additional or corrected information to issuing body"@en-AU ;
    skos:narrower F2021L00315:32 ;
    skos:prefLabel "Item I33"@en-AU ;
    dcat:accessURL <https://www.legislation.gov.au/F2021L00315/2023-08-04/2023-08-04/text/original/epub/OEBPS/document_1/document_1.html#_Toc143853857> ;
    dcat:landingPage "https://www.legislation.gov.au/F2021L00315/2023-08-04/2023-08-04/text/original/epub/OEBPS/document_1/document_1.html#_Toc143853857"^^xsd:anyURI ;
    dcat:theme legcons:Item .

F2021L00315:34 a legcons:Item,
        owl:Class,
        dcat:Resource ;
    rdfs:label "Item - I34 2 15  Circumstances for refusing to issue government certificate"@en-AU ;
    dct:isPartOf F2021L00315:32 ;
    dct:isReferencedBy F2021L00315: ;
    rdfs:comment "2 15  Circumstances for refusing to issue government certificate - Abrievated Graph Key: I34"@en-AU ;
    skos:definition "2 15  Circumstances for refusing to issue government certificate"@en-AU ;
    skos:narrower F2021L00315:32 ;
    skos:prefLabel "Item I34"@en-AU ;
    dcat:accessURL <https://www.legislation.gov.au/F2021L00315/2023-08-04/2023-08-04/text/original/epub/OEBPS/document_1/document_1.html#_Toc143853858> ;
    dcat:landingPage "https://www.legislation.gov.au/F2021L00315/2023-08-04/2023-08-04/text/original/epub/OEBPS/document_1/document_1.html#_Toc143853858"^^xsd:anyURI ;
    dcat:theme legcons:Item .

F2021L00315:36 a legcons:Item,
        owl:Class,
        dcat:Resource ;
    rdfs:label "Item - I36 2 16  Changes that require holder of government certificate to give additional or corrected information to issuing body"@en-AU ;
    dct:isPartOf F2021L00315:35 ;
    dct:isReferencedBy F2021L00315: ;
    rdfs:comment "2 16  Changes that require holder of government certificate to give additional or corrected information to issuing body - Abrievated Graph Key: I36"@en-AU ;
    skos:definition "2 16  Changes that require holder of government certificate to give additional or corrected information to issuing body"@en-AU ;
    skos:narrower F2021L00315:35 ;
    skos:prefLabel "Item I36"@en-AU ;
    dcat:accessURL <https://www.legislation.gov.au/F2021L00315/2023-08-04/2023-08-04/text/original/epub/OEBPS/document_1/document_1.html#_Toc143853860> ;
    dcat:landingPage "https://www.legislation.gov.au/F2021L00315/2023-08-04/2023-08-04/text/original/epub/OEBPS/document_1/document_1.html#_Toc143853860"^^xsd:anyURI ;
    dcat:theme legcons:Item .

F2021L00315:39 a legcons:Item,
        owl:Class,
        dcat:Resource ;
    rdfs:label "Item - I39 3 1  Other requirements for accreditation"@en-AU ;
    dct:isPartOf F2021L00315:38 ;
    dct:isReferencedBy F2021L00315: ;
    rdfs:comment "3 1  Other requirements for accreditation - Abrievated Graph Key: I39"@en-AU ;
    skos:definition "3 1  Other requirements for accreditation"@en-AU ;
    skos:narrower F2021L00315:38 ;
    skos:prefLabel "Item I39"@en-AU ;
    dcat:accessURL <https://www.legislation.gov.au/F2021L00315/2023-08-04/2023-08-04/text/original/epub/OEBPS/document_1/document_1.html#_Toc143853863> ;
    dcat:landingPage "https://www.legislation.gov.au/F2021L00315/2023-08-04/2023-08-04/text/original/epub/OEBPS/document_1/document_1.html#_Toc143853863"^^xsd:anyURI ;
    dcat:theme legcons:Item .

F2021L00315:4 a legcons:Item,
        owl:Class,
        dcat:Resource ;
    rdfs:label "Item - I4 1 3  Authority"@en-AU ;
    dct:isPartOf F2021L00315:1 ;
    dct:isReferencedBy F2021L00315: ;
    rdfs:comment "1 3  Authority - Abrievated Graph Key: I4"@en-AU ;
    skos:definition "1 3  Authority"@en-AU ;
    skos:narrower F2021L00315:1 ;
    skos:prefLabel "Item I4"@en-AU ;
    dcat:accessURL <https://www.legislation.gov.au/F2021L00315/2023-08-04/2023-08-04/text/original/epub/OEBPS/document_1/document_1.html#_Toc143853828> ;
    dcat:landingPage "https://www.legislation.gov.au/F2021L00315/2023-08-04/2023-08-04/text/original/epub/OEBPS/document_1/document_1.html#_Toc143853828"^^xsd:anyURI ;
    dcat:theme legcons:Item .

F2021L00315:41 a legcons:Item,
        owl:Class,
        dcat:Resource ;
    rdfs:label "Item - I41 3 2  Purpose of this Part"@en-AU ;
    dct:isPartOf F2021L00315:40 ;
    dct:isReferencedBy F2021L00315: ;
    rdfs:comment "3 2  Purpose of this Part - Abrievated Graph Key: I41"@en-AU ;
    skos:definition "3 2  Purpose of this Part"@en-AU ;
    skos:narrower F2021L00315:40 ;
    skos:prefLabel "Item I41"@en-AU ;
    dcat:accessURL <https://www.legislation.gov.au/F2021L00315/2023-08-04/2023-08-04/text/original/epub/OEBPS/document_1/document_1.html#_Toc143853865> ;
    dcat:landingPage "https://www.legislation.gov.au/F2021L00315/2023-08-04/2023-08-04/text/original/epub/OEBPS/document_1/document_1.html#_Toc143853865"^^xsd:anyURI ;
    dcat:theme legcons:Item .

F2021L00315:42 a legcons:Item,
        owl:Class,
        dcat:Resource ;
    rdfs:label "Item - I42 3 3  Importing country requirements must be met"@en-AU ;
    dct:isPartOf F2021L00315:40 ;
    dct:isReferencedBy F2021L00315: ;
    rdfs:comment "3 3  Importing country requirements must be met - Abrievated Graph Key: I42"@en-AU ;
    skos:definition "3 3  Importing country requirements must be met"@en-AU ;
    skos:narrower F2021L00315:40 ;
    skos:prefLabel "Item I42"@en-AU ;
    dcat:accessURL <https://www.legislation.gov.au/F2021L00315/2023-08-04/2023-08-04/text/original/epub/OEBPS/document_1/document_1.html#_Toc143853866> ;
    dcat:landingPage "https://www.legislation.gov.au/F2021L00315/2023-08-04/2023-08-04/text/original/epub/OEBPS/document_1/document_1.html#_Toc143853866"^^xsd:anyURI ;
    dcat:theme legcons:Item .

F2021L00315:43 a legcons:Item,
        owl:Class,
        dcat:Resource ;
    rdfs:label "Item - I43 3 3 A  Property must be kept in appropriate condition"@en-AU ;
    dct:isPartOf F2021L00315:40 ;
    dct:isReferencedBy F2021L00315: ;
    rdfs:comment "3 3 A  Property must be kept in appropriate condition - Abrievated Graph Key: I43"@en-AU ;
    skos:definition "3 3 A  Property must be kept in appropriate condition"@en-AU ;
    skos:narrower F2021L00315:40 ;
    skos:prefLabel "Item I43"@en-AU ;
    dcat:accessURL <https://www.legislation.gov.au/F2021L00315/2023-08-04/2023-08-04/text/original/epub/OEBPS/document_1/document_1.html#_Toc143853867> ;
    dcat:landingPage "https://www.legislation.gov.au/F2021L00315/2023-08-04/2023-08-04/text/original/epub/OEBPS/document_1/document_1.html#_Toc143853867"^^xsd:anyURI ;
    dcat:theme legcons:Item .

F2021L00315:44 a legcons:Item,
        owl:Class,
        dcat:Resource ;
    rdfs:label "Item - I44 3 3 B  Plants and plant products must be traced"@en-AU ;
    dct:isPartOf F2021L00315:40 ;
    dct:isReferencedBy F2021L00315: ;
    rdfs:comment "3 3 B  Plants and plant products must be traced - Abrievated Graph Key: I44"@en-AU ;
    skos:definition "3 3 B  Plants and plant products must be traced"@en-AU ;
    skos:narrower F2021L00315:40 ;
    skos:prefLabel "Item I44"@en-AU ;
    dcat:accessURL <https://www.legislation.gov.au/F2021L00315/2023-08-04/2023-08-04/text/original/epub/OEBPS/document_1/document_1.html#_Toc143853868> ;
    dcat:landingPage "https://www.legislation.gov.au/F2021L00315/2023-08-04/2023-08-04/text/original/epub/OEBPS/document_1/document_1.html#_Toc143853868"^^xsd:anyURI ;
    dcat:theme legcons:Item .

F2021L00315:45 a legcons:Item,
        owl:Class,
        dcat:Resource ;
    rdfs:label "Item - I45 3 4  Integrity"@en-AU ;
    dct:isPartOf F2021L00315:40 ;
    dct:isReferencedBy F2021L00315: ;
    rdfs:comment "3 4  Integrity - Abrievated Graph Key: I45"@en-AU ;
    skos:definition "3 4  Integrity"@en-AU ;
    skos:narrower F2021L00315:40 ;
    skos:prefLabel "Item I45"@en-AU ;
    dcat:accessURL <https://www.legislation.gov.au/F2021L00315/2023-08-04/2023-08-04/text/original/epub/OEBPS/document_1/document_1.html#_Toc143853869> ;
    dcat:landingPage "https://www.legislation.gov.au/F2021L00315/2023-08-04/2023-08-04/text/original/epub/OEBPS/document_1/document_1.html#_Toc143853869"^^xsd:anyURI ;
    dcat:theme legcons:Item .

F2021L00315:46 a legcons:Item,
        owl:Class,
        dcat:Resource ;
    rdfs:label "Item - I46 3 5  Application of trade description"@en-AU ;
    dct:isPartOf F2021L00315:40 ;
    dct:isReferencedBy F2021L00315: ;
    rdfs:comment "3 5  Application of trade description - Abrievated Graph Key: I46"@en-AU ;
    skos:definition "3 5  Application of trade description"@en-AU ;
    skos:narrower F2021L00315:40 ;
    skos:prefLabel "Item I46"@en-AU ;
    dcat:accessURL <https://www.legislation.gov.au/F2021L00315/2023-08-04/2023-08-04/text/original/epub/OEBPS/document_1/document_1.html#_Toc143853870> ;
    dcat:landingPage "https://www.legislation.gov.au/F2021L00315/2023-08-04/2023-08-04/text/original/epub/OEBPS/document_1/document_1.html#_Toc143853870"^^xsd:anyURI ;
    dcat:theme legcons:Item .

F2021L00315:47 a legcons:Item,
        owl:Class,
        dcat:Resource ;
    rdfs:label "Item - I47 3 6  Requirements for packages for export"@en-AU ;
    dct:isPartOf F2021L00315:40 ;
    dct:isReferencedBy F2021L00315: ;
    rdfs:comment "3 6  Requirements for packages for export - Abrievated Graph Key: I47"@en-AU ;
    skos:definition "3 6  Requirements for packages for export"@en-AU ;
    skos:narrower F2021L00315:40 ;
    skos:prefLabel "Item I47"@en-AU ;
    dcat:accessURL <https://www.legislation.gov.au/F2021L00315/2023-08-04/2023-08-04/text/original/epub/OEBPS/document_1/document_1.html#_Toc143853871> ;
    dcat:landingPage "https://www.legislation.gov.au/F2021L00315/2023-08-04/2023-08-04/text/original/epub/OEBPS/document_1/document_1.html#_Toc143853871"^^xsd:anyURI ;
    dcat:theme legcons:Item .

F2021L00315:49 a legcons:Item,
        owl:Class,
        dcat:Resource ;
    rdfs:label "Item - I49 3 7  Period within which application to renew accreditation must be made"@en-AU ;
    dct:isPartOf F2021L00315:48 ;
    dct:isReferencedBy F2021L00315: ;
    rdfs:comment "3 7  Period within which application to renew accreditation must be made - Abrievated Graph Key: I49"@en-AU ;
    skos:definition "3 7  Period within which application to renew accreditation must be made"@en-AU ;
    skos:narrower F2021L00315:48 ;
    skos:prefLabel "Item I49"@en-AU ;
    dcat:accessURL <https://www.legislation.gov.au/F2021L00315/2023-08-04/2023-08-04/text/original/epub/OEBPS/document_1/document_1.html#_Toc143853873> ;
    dcat:landingPage "https://www.legislation.gov.au/F2021L00315/2023-08-04/2023-08-04/text/original/epub/OEBPS/document_1/document_1.html#_Toc143853873"^^xsd:anyURI ;
    dcat:theme legcons:Item .

F2021L00315:5 a legcons:Item,
        owl:Class,
        dcat:Resource ;
    rdfs:label "Item - I5 1 4  Extension of the Act to Norfolk Island"@en-AU ;
    dct:isPartOf F2021L00315:1 ;
    dct:isReferencedBy F2021L00315: ;
    rdfs:comment "1 4  Extension of the Act to Norfolk Island - Abrievated Graph Key: I5"@en-AU ;
    skos:definition "1 4  Extension of the Act to Norfolk Island"@en-AU ;
    skos:narrower F2021L00315:1 ;
    skos:prefLabel "Item I5"@en-AU ;
    dcat:accessURL <https://www.legislation.gov.au/F2021L00315/2023-08-04/2023-08-04/text/original/epub/OEBPS/document_1/document_1.html#_Toc143853829> ;
    dcat:landingPage "https://www.legislation.gov.au/F2021L00315/2023-08-04/2023-08-04/text/original/epub/OEBPS/document_1/document_1.html#_Toc143853829"^^xsd:anyURI ;
    dcat:theme legcons:Item .

F2021L00315:50 a legcons:Item,
        owl:Class,
        dcat:Resource ;
    rdfs:label "Item - I50 3 8  Conditions of renewed accreditation"@en-AU ;
    dct:isPartOf F2021L00315:48 ;
    dct:isReferencedBy F2021L00315: ;
    rdfs:comment "3 8  Conditions of renewed accreditation - Abrievated Graph Key: I50"@en-AU ;
    skos:definition "3 8  Conditions of renewed accreditation"@en-AU ;
    skos:narrower F2021L00315:48 ;
    skos:prefLabel "Item I50"@en-AU ;
    dcat:accessURL <https://www.legislation.gov.au/F2021L00315/2023-08-04/2023-08-04/text/original/epub/OEBPS/document_1/document_1.html#_Toc143853874> ;
    dcat:landingPage "https://www.legislation.gov.au/F2021L00315/2023-08-04/2023-08-04/text/original/epub/OEBPS/document_1/document_1.html#_Toc143853874"^^xsd:anyURI ;
    dcat:theme legcons:Item .

F2021L00315:52 a legcons:Item,
        owl:Class,
        dcat:Resource ;
    rdfs:label "Item - I52 3 9  Alterations of property that must be approved"@en-AU ;
    dct:isPartOf F2021L00315:51 ;
    dct:isReferencedBy F2021L00315: ;
    rdfs:comment "3 9  Alterations of property that must be approved - Abrievated Graph Key: I52"@en-AU ;
    skos:definition "3 9  Alterations of property that must be approved"@en-AU ;
    skos:narrower F2021L00315:51 ;
    skos:prefLabel "Item I52"@en-AU ;
    dcat:accessURL <https://www.legislation.gov.au/F2021L00315/2023-08-04/2023-08-04/text/original/epub/OEBPS/document_1/document_1.html#_Toc143853876> ;
    dcat:landingPage "https://www.legislation.gov.au/F2021L00315/2023-08-04/2023-08-04/text/original/epub/OEBPS/document_1/document_1.html#_Toc143853876"^^xsd:anyURI ;
    dcat:theme legcons:Item .

F2021L00315:53 a legcons:Item,
        owl:Class,
        dcat:Resource ;
    rdfs:label "Item - I53 3 10  Other reasons for Secretary to make variation in relation to accreditation"@en-AU ;
    dct:isPartOf F2021L00315:51 ;
    dct:isReferencedBy F2021L00315: ;
    rdfs:comment "3 10  Other reasons for Secretary to make variation in relation to accreditation - Abrievated Graph Key: I53"@en-AU ;
    skos:definition "3 10  Other reasons for Secretary to make variation in relation to accreditation"@en-AU ;
    skos:narrower F2021L00315:51 ;
    skos:prefLabel "Item I53"@en-AU ;
    dcat:accessURL <https://www.legislation.gov.au/F2021L00315/2023-08-04/2023-08-04/text/original/epub/OEBPS/document_1/document_1.html#_Toc143853877> ;
    dcat:landingPage "https://www.legislation.gov.au/F2021L00315/2023-08-04/2023-08-04/text/original/epub/OEBPS/document_1/document_1.html#_Toc143853877"^^xsd:anyURI ;
    dcat:theme legcons:Item .

F2021L00315:56 a legcons:Item,
        owl:Class,
        dcat:Resource ;
    rdfs:label "Item - I56 3 11  Circumstances in which manager may request suspension of accreditation"@en-AU ;
    dct:isPartOf F2021L00315:55 ;
    dct:isReferencedBy F2021L00315: ;
    rdfs:comment "3 11  Circumstances in which manager may request suspension of accreditation - Abrievated Graph Key: I56"@en-AU ;
    skos:definition "3 11  Circumstances in which manager may request suspension of accreditation"@en-AU ;
    skos:narrower F2021L00315:55 ;
    skos:prefLabel "Item I56"@en-AU ;
    dcat:accessURL <https://www.legislation.gov.au/F2021L00315/2023-08-04/2023-08-04/text/original/epub/OEBPS/document_1/document_1.html#_Toc143853880> ;
    dcat:landingPage "https://www.legislation.gov.au/F2021L00315/2023-08-04/2023-08-04/text/original/epub/OEBPS/document_1/document_1.html#_Toc143853880"^^xsd:anyURI ;
    dcat:theme legcons:Item .

F2021L00315:58 a legcons:Item,
        owl:Class,
        dcat:Resource ;
    rdfs:label "Item - I58 3 12  Other grounds for suspension of accreditation"@en-AU ;
    dct:isPartOf F2021L00315:57 ;
    dct:isReferencedBy F2021L00315: ;
    rdfs:comment "3 12  Other grounds for suspension of accreditation - Abrievated Graph Key: I58"@en-AU ;
    skos:definition "3 12  Other grounds for suspension of accreditation"@en-AU ;
    skos:narrower F2021L00315:57 ;
    skos:prefLabel "Item I58"@en-AU ;
    dcat:accessURL <https://www.legislation.gov.au/F2021L00315/2023-08-04/2023-08-04/text/original/epub/OEBPS/document_1/document_1.html#_Toc143853882> ;
    dcat:landingPage "https://www.legislation.gov.au/F2021L00315/2023-08-04/2023-08-04/text/original/epub/OEBPS/document_1/document_1.html#_Toc143853882"^^xsd:anyURI ;
    dcat:theme legcons:Item .

F2021L00315:6 a legcons:Item,
        owl:Class,
        dcat:Resource ;
    rdfs:label "Item - I6 1 5  Simplified outline of this instrument"@en-AU ;
    dct:isPartOf F2021L00315:1 ;
    dct:isReferencedBy F2021L00315: ;
    rdfs:comment "1 5  Simplified outline of this instrument - Abrievated Graph Key: I6"@en-AU ;
    skos:definition "1 5  Simplified outline of this instrument"@en-AU ;
    skos:narrower F2021L00315:1 ;
    skos:prefLabel "Item I6"@en-AU ;
    dcat:accessURL <https://www.legislation.gov.au/F2021L00315/2023-08-04/2023-08-04/text/original/epub/OEBPS/document_1/document_1.html#_Toc143853830> ;
    dcat:landingPage "https://www.legislation.gov.au/F2021L00315/2023-08-04/2023-08-04/text/original/epub/OEBPS/document_1/document_1.html#_Toc143853830"^^xsd:anyURI ;
    dcat:theme legcons:Item .

F2021L00315:61 a legcons:Item,
        owl:Class,
        dcat:Resource ;
    rdfs:label "Item - I61 3 13  Information to be included in request to revoke accreditation"@en-AU ;
    dct:isPartOf F2021L00315:60 ;
    dct:isReferencedBy F2021L00315: ;
    rdfs:comment "3 13  Information to be included in request to revoke accreditation - Abrievated Graph Key: I61"@en-AU ;
    skos:definition "3 13  Information to be included in request to revoke accreditation"@en-AU ;
    skos:narrower F2021L00315:60 ;
    skos:prefLabel "Item I61"@en-AU ;
    dcat:accessURL <https://www.legislation.gov.au/F2021L00315/2023-08-04/2023-08-04/text/original/epub/OEBPS/document_1/document_1.html#_Toc143853885> ;
    dcat:landingPage "https://www.legislation.gov.au/F2021L00315/2023-08-04/2023-08-04/text/original/epub/OEBPS/document_1/document_1.html#_Toc143853885"^^xsd:anyURI ;
    dcat:theme legcons:Item .

F2021L00315:63 a legcons:Item,
        owl:Class,
        dcat:Resource ;
    rdfs:label "Item - I63 3 14  Other grounds for revocation of accreditation"@en-AU ;
    dct:isPartOf F2021L00315:62 ;
    dct:isReferencedBy F2021L00315: ;
    rdfs:comment "3 14  Other grounds for revocation of accreditation - Abrievated Graph Key: I63"@en-AU ;
    skos:definition "3 14  Other grounds for revocation of accreditation"@en-AU ;
    skos:narrower F2021L00315:62 ;
    skos:prefLabel "Item I63"@en-AU ;
    dcat:accessURL <https://www.legislation.gov.au/F2021L00315/2023-08-04/2023-08-04/text/original/epub/OEBPS/document_1/document_1.html#_Toc143853887> ;
    dcat:landingPage "https://www.legislation.gov.au/F2021L00315/2023-08-04/2023-08-04/text/original/epub/OEBPS/document_1/document_1.html#_Toc143853887"^^xsd:anyURI ;
    dcat:theme legcons:Item .

F2021L00315:65 a legcons:Item,
        owl:Class,
        dcat:Resource ;
    rdfs:label "Item - I65 3 15  Events of which Secretary must be notified"@en-AU ;
    dct:isPartOf F2021L00315:64 ;
    dct:isReferencedBy F2021L00315: ;
    rdfs:comment "3 15  Events of which Secretary must be notified - Abrievated Graph Key: I65"@en-AU ;
    skos:definition "3 15  Events of which Secretary must be notified"@en-AU ;
    skos:narrower F2021L00315:64 ;
    skos:prefLabel "Item I65"@en-AU ;
    dcat:accessURL <https://www.legislation.gov.au/F2021L00315/2023-08-04/2023-08-04/text/original/epub/OEBPS/document_1/document_1.html#_Toc143853889> ;
    dcat:landingPage "https://www.legislation.gov.au/F2021L00315/2023-08-04/2023-08-04/text/original/epub/OEBPS/document_1/document_1.html#_Toc143853889"^^xsd:anyURI ;
    dcat:theme legcons:Item .

F2021L00315:67 a legcons:Item,
        owl:Class,
        dcat:Resource ;
    rdfs:label "Item - I67 3 16  Application of this Part"@en-AU ;
    dct:isPartOf F2021L00315:66 ;
    dct:isReferencedBy F2021L00315: ;
    rdfs:comment "3 16  Application of this Part - Abrievated Graph Key: I67"@en-AU ;
    skos:definition "3 16  Application of this Part"@en-AU ;
    skos:narrower F2021L00315:66 ;
    skos:prefLabel "Item I67"@en-AU ;
    dcat:accessURL <https://www.legislation.gov.au/F2021L00315/2023-08-04/2023-08-04/text/original/epub/OEBPS/document_1/document_1.html#_Toc143853891> ;
    dcat:landingPage "https://www.legislation.gov.au/F2021L00315/2023-08-04/2023-08-04/text/original/epub/OEBPS/document_1/document_1.html#_Toc143853891"^^xsd:anyURI ;
    dcat:theme legcons:Item .

F2021L00315:68 a legcons:Item,
        owl:Class,
        dcat:Resource ;
    rdfs:label "Item - I68 3 17  Initial consideration period"@en-AU ;
    dct:isPartOf F2021L00315:66 ;
    dct:isReferencedBy F2021L00315: ;
    rdfs:comment "3 17  Initial consideration period - Abrievated Graph Key: I68"@en-AU ;
    skos:definition "3 17  Initial consideration period"@en-AU ;
    skos:narrower F2021L00315:66 ;
    skos:prefLabel "Item I68"@en-AU ;
    dcat:accessURL <https://www.legislation.gov.au/F2021L00315/2023-08-04/2023-08-04/text/original/epub/OEBPS/document_1/document_1.html#_Toc143853892> ;
    dcat:landingPage "https://www.legislation.gov.au/F2021L00315/2023-08-04/2023-08-04/text/original/epub/OEBPS/document_1/document_1.html#_Toc143853892"^^xsd:anyURI ;
    dcat:theme legcons:Item .

F2021L00315:69 a legcons:Item,
        owl:Class,
        dcat:Resource ;
    rdfs:label "Item - I69 3 18  Period within which request relating to application must be complied with"@en-AU ;
    dct:isPartOf F2021L00315:66 ;
    dct:isReferencedBy F2021L00315: ;
    rdfs:comment "3 18  Period within which request relating to application must be complied with - Abrievated Graph Key: I69"@en-AU ;
    skos:definition "3 18  Period within which request relating to application must be complied with"@en-AU ;
    skos:narrower F2021L00315:66 ;
    skos:prefLabel "Item I69"@en-AU ;
    dcat:accessURL <https://www.legislation.gov.au/F2021L00315/2023-08-04/2023-08-04/text/original/epub/OEBPS/document_1/document_1.html#_Toc143853893> ;
    dcat:landingPage "https://www.legislation.gov.au/F2021L00315/2023-08-04/2023-08-04/text/original/epub/OEBPS/document_1/document_1.html#_Toc143853893"^^xsd:anyURI ;
    dcat:theme legcons:Item .

F2021L00315:7 a legcons:Part,
        owl:Class,
        dcat:Resource ;
    rdfs:label "Part - P7 Part 2 Interpretation"@en-AU ;
    dct:isPartOf F2021L00315:1 ;
    dct:isReferencedBy F2021L00315: ;
    rdfs:comment "Part 2 Interpretation - Abrievated Graph Key: P7"@en-AU ;
    skos:definition "Part 2 Interpretation"@en-AU ;
    skos:narrower F2021L00315:1 ;
    skos:prefLabel "Part P7"@en-AU ;
    dcat:accessURL <https://www.legislation.gov.au/F2021L00315/2023-08-04/2023-08-04/text/original/epub/OEBPS/document_1/document_1.html#_Toc143853831> ;
    dcat:landingPage "https://www.legislation.gov.au/F2021L00315/2023-08-04/2023-08-04/text/original/epub/OEBPS/document_1/document_1.html#_Toc143853831"^^xsd:anyURI ;
    dcat:theme legcons:Part .

F2021L00315:72 a legcons:Item,
        owl:Class,
        dcat:Resource ;
    rdfs:label "Item - I72 4 1  Purpose of this Part"@en-AU ;
    dct:isPartOf F2021L00315:71 ;
    dct:isReferencedBy F2021L00315: ;
    rdfs:comment "4 1  Purpose of this Part - Abrievated Graph Key: I72"@en-AU ;
    skos:definition "4 1  Purpose of this Part"@en-AU ;
    skos:narrower F2021L00315:71 ;
    skos:prefLabel "Item I72"@en-AU ;
    dcat:accessURL <https://www.legislation.gov.au/F2021L00315/2023-08-04/2023-08-04/text/original/epub/OEBPS/document_1/document_1.html#_Toc143853896> ;
    dcat:landingPage "https://www.legislation.gov.au/F2021L00315/2023-08-04/2023-08-04/text/original/epub/OEBPS/document_1/document_1.html#_Toc143853896"^^xsd:anyURI ;
    dcat:theme legcons:Item .

F2021L00315:73 a legcons:Item,
        owl:Class,
        dcat:Resource ;
    rdfs:label "Item - I73 4 2  Construction equipment and facilities"@en-AU ;
    dct:isPartOf F2021L00315:71 ;
    dct:isReferencedBy F2021L00315: ;
    rdfs:comment "4 2  Construction equipment and facilities - Abrievated Graph Key: I73"@en-AU ;
    skos:definition "4 2  Construction equipment and facilities"@en-AU ;
    skos:narrower F2021L00315:71 ;
    skos:prefLabel "Item I73"@en-AU ;
    dcat:accessURL <https://www.legislation.gov.au/F2021L00315/2023-08-04/2023-08-04/text/original/epub/OEBPS/document_1/document_1.html#_Toc143853897> ;
    dcat:landingPage "https://www.legislation.gov.au/F2021L00315/2023-08-04/2023-08-04/text/original/epub/OEBPS/document_1/document_1.html#_Toc143853897"^^xsd:anyURI ;
    dcat:theme legcons:Item .

F2021L00315:74 a legcons:Item,
        owl:Class,
        dcat:Resource ;
    rdfs:label "Item - I74 4 3  Other requirements"@en-AU ;
    dct:isPartOf F2021L00315:71 ;
    dct:isReferencedBy F2021L00315: ;
    rdfs:comment "4 3  Other requirements - Abrievated Graph Key: I74"@en-AU ;
    skos:definition "4 3  Other requirements"@en-AU ;
    skos:narrower F2021L00315:71 ;
    skos:prefLabel "Item I74"@en-AU ;
    dcat:accessURL <https://www.legislation.gov.au/F2021L00315/2023-08-04/2023-08-04/text/original/epub/OEBPS/document_1/document_1.html#_Toc143853898> ;
    dcat:landingPage "https://www.legislation.gov.au/F2021L00315/2023-08-04/2023-08-04/text/original/epub/OEBPS/document_1/document_1.html#_Toc143853898"^^xsd:anyURI ;
    dcat:theme legcons:Item .

F2021L00315:76 a legcons:Item,
        owl:Class,
        dcat:Resource ;
    rdfs:label "Item - I76 4 5  Purpose of this Part"@en-AU ;
    dct:isPartOf F2021L00315:75 ;
    dct:isReferencedBy F2021L00315: ;
    rdfs:comment "4 5  Purpose of this Part - Abrievated Graph Key: I76"@en-AU ;
    skos:definition "4 5  Purpose of this Part"@en-AU ;
    skos:narrower F2021L00315:75 ;
    skos:prefLabel "Item I76"@en-AU ;
    dcat:accessURL <https://www.legislation.gov.au/F2021L00315/2023-08-04/2023-08-04/text/original/epub/OEBPS/document_1/document_1.html#_Toc143853900> ;
    dcat:landingPage "https://www.legislation.gov.au/F2021L00315/2023-08-04/2023-08-04/text/original/epub/OEBPS/document_1/document_1.html#_Toc143853900"^^xsd:anyURI ;
    dcat:theme legcons:Item .

F2021L00315:77 a legcons:Item,
        owl:Class,
        dcat:Resource ;
    rdfs:label "Item - I77 4 6  Construction equipment and facilities"@en-AU ;
    dct:isPartOf F2021L00315:75 ;
    dct:isReferencedBy F2021L00315: ;
    rdfs:comment "4 6  Construction equipment and facilities - Abrievated Graph Key: I77"@en-AU ;
    skos:definition "4 6  Construction equipment and facilities"@en-AU ;
    skos:narrower F2021L00315:75 ;
    skos:prefLabel "Item I77"@en-AU ;
    dcat:accessURL <https://www.legislation.gov.au/F2021L00315/2023-08-04/2023-08-04/text/original/epub/OEBPS/document_1/document_1.html#_Toc143853901> ;
    dcat:landingPage "https://www.legislation.gov.au/F2021L00315/2023-08-04/2023-08-04/text/original/epub/OEBPS/document_1/document_1.html#_Toc143853901"^^xsd:anyURI ;
    dcat:theme legcons:Item .

F2021L00315:78 a legcons:Item,
        owl:Class,
        dcat:Resource ;
    rdfs:label "Item - I78 4 7  Importing country requirements must be met"@en-AU ;
    dct:isPartOf F2021L00315:75 ;
    dct:isReferencedBy F2021L00315: ;
    rdfs:comment "4 7  Importing country requirements must be met - Abrievated Graph Key: I78"@en-AU ;
    skos:definition "4 7  Importing country requirements must be met"@en-AU ;
    skos:narrower F2021L00315:75 ;
    skos:prefLabel "Item I78"@en-AU ;
    dcat:accessURL <https://www.legislation.gov.au/F2021L00315/2023-08-04/2023-08-04/text/original/epub/OEBPS/document_1/document_1.html#_Toc143853902> ;
    dcat:landingPage "https://www.legislation.gov.au/F2021L00315/2023-08-04/2023-08-04/text/original/epub/OEBPS/document_1/document_1.html#_Toc143853902"^^xsd:anyURI ;
    dcat:theme legcons:Item .

F2021L00315:79 a legcons:Item,
        owl:Class,
        dcat:Resource ;
    rdfs:label "Item - I79 4 7 A  Establishment must be kept in appropriate condition"@en-AU ;
    dct:isPartOf F2021L00315:75 ;
    dct:isReferencedBy F2021L00315: ;
    rdfs:comment "4 7 A  Establishment must be kept in appropriate condition - Abrievated Graph Key: I79"@en-AU ;
    skos:definition "4 7 A  Establishment must be kept in appropriate condition"@en-AU ;
    skos:narrower F2021L00315:75 ;
    skos:prefLabel "Item I79"@en-AU ;
    dcat:accessURL <https://www.legislation.gov.au/F2021L00315/2023-08-04/2023-08-04/text/original/epub/OEBPS/document_1/document_1.html#_Toc143853903> ;
    dcat:landingPage "https://www.legislation.gov.au/F2021L00315/2023-08-04/2023-08-04/text/original/epub/OEBPS/document_1/document_1.html#_Toc143853903"^^xsd:anyURI ;
    dcat:theme legcons:Item .

F2021L00315:8 a legcons:Item,
        owl:Class,
        dcat:Resource ;
    rdfs:label "Item - I8 1 6  Definitions"@en-AU ;
    dct:isPartOf F2021L00315:1 ;
    dct:isReferencedBy F2021L00315: ;
    rdfs:comment "1 6  Definitions - Abrievated Graph Key: I8"@en-AU ;
    skos:definition "1 6  Definitions"@en-AU ;
    skos:narrower F2021L00315:1 ;
    skos:prefLabel "Item I8"@en-AU ;
    dcat:accessURL <https://www.legislation.gov.au/F2021L00315/2023-08-04/2023-08-04/text/original/epub/OEBPS/document_1/document_1.html#_Toc143853832> ;
    dcat:landingPage "https://www.legislation.gov.au/F2021L00315/2023-08-04/2023-08-04/text/original/epub/OEBPS/document_1/document_1.html#_Toc143853832"^^xsd:anyURI ;
    dcat:theme legcons:Item .

F2021L00315:80 a legcons:Item,
        owl:Class,
        dcat:Resource ;
    rdfs:label "Item - I80 4 7 B  Plants and plant products must be traced"@en-AU ;
    dct:isPartOf F2021L00315:75 ;
    dct:isReferencedBy F2021L00315: ;
    rdfs:comment "4 7 B  Plants and plant products must be traced - Abrievated Graph Key: I80"@en-AU ;
    skos:definition "4 7 B  Plants and plant products must be traced"@en-AU ;
    skos:narrower F2021L00315:75 ;
    skos:prefLabel "Item I80"@en-AU ;
    dcat:accessURL <https://www.legislation.gov.au/F2021L00315/2023-08-04/2023-08-04/text/original/epub/OEBPS/document_1/document_1.html#_Toc143853904> ;
    dcat:landingPage "https://www.legislation.gov.au/F2021L00315/2023-08-04/2023-08-04/text/original/epub/OEBPS/document_1/document_1.html#_Toc143853904"^^xsd:anyURI ;
    dcat:theme legcons:Item .

F2021L00315:81 a legcons:Item,
        owl:Class,
        dcat:Resource ;
    rdfs:label "Item - I81 4 8  Integrity"@en-AU ;
    dct:isPartOf F2021L00315:75 ;
    dct:isReferencedBy F2021L00315: ;
    rdfs:comment "4 8  Integrity - Abrievated Graph Key: I81"@en-AU ;
    skos:definition "4 8  Integrity"@en-AU ;
    skos:narrower F2021L00315:75 ;
    skos:prefLabel "Item I81"@en-AU ;
    dcat:accessURL <https://www.legislation.gov.au/F2021L00315/2023-08-04/2023-08-04/text/original/epub/OEBPS/document_1/document_1.html#_Toc143853905> ;
    dcat:landingPage "https://www.legislation.gov.au/F2021L00315/2023-08-04/2023-08-04/text/original/epub/OEBPS/document_1/document_1.html#_Toc143853905"^^xsd:anyURI ;
    dcat:theme legcons:Item .

F2021L00315:82 a legcons:Item,
        owl:Class,
        dcat:Resource ;
    rdfs:label "Item - I82 4 8 A  Conditions relating to treatment of prescribed plants or plant products"@en-AU ;
    dct:isPartOf F2021L00315:75 ;
    dct:isReferencedBy F2021L00315: ;
    rdfs:comment "4 8 A  Conditions relating to treatment of prescribed plants or plant products - Abrievated Graph Key: I82"@en-AU ;
    skos:definition "4 8 A  Conditions relating to treatment of prescribed plants or plant products"@en-AU ;
    skos:narrower F2021L00315:75 ;
    skos:prefLabel "Item I82"@en-AU ;
    dcat:accessURL <https://www.legislation.gov.au/F2021L00315/2023-08-04/2023-08-04/text/original/epub/OEBPS/document_1/document_1.html#_Toc143853906> ;
    dcat:landingPage "https://www.legislation.gov.au/F2021L00315/2023-08-04/2023-08-04/text/original/epub/OEBPS/document_1/document_1.html#_Toc143853906"^^xsd:anyURI ;
    dcat:theme legcons:Item .

F2021L00315:83 a legcons:Item,
        owl:Class,
        dcat:Resource ;
    rdfs:label "Item - I83 4 9  Conditions relating to prescribed grain etc"@en-AU ;
    dct:isPartOf F2021L00315:75 ;
    dct:isReferencedBy F2021L00315: ;
    rdfs:comment "4 9  Conditions relating to prescribed grain etc - Abrievated Graph Key: I83"@en-AU ;
    skos:definition "4 9  Conditions relating to prescribed grain etc"@en-AU ;
    skos:narrower F2021L00315:75 ;
    skos:prefLabel "Item I83"@en-AU ;
    dcat:accessURL <https://www.legislation.gov.au/F2021L00315/2023-08-04/2023-08-04/text/original/epub/OEBPS/document_1/document_1.html#_Toc143853907> ;
    dcat:landingPage "https://www.legislation.gov.au/F2021L00315/2023-08-04/2023-08-04/text/original/epub/OEBPS/document_1/document_1.html#_Toc143853907"^^xsd:anyURI ;
    dcat:theme legcons:Item .

F2021L00315:84 a legcons:Item,
        owl:Class,
        dcat:Resource ;
    rdfs:label "Item - I84 4 10  Application of trade description"@en-AU ;
    dct:isPartOf F2021L00315:75 ;
    dct:isReferencedBy F2021L00315: ;
    rdfs:comment "4 10  Application of trade description - Abrievated Graph Key: I84"@en-AU ;
    skos:definition "4 10  Application of trade description"@en-AU ;
    skos:narrower F2021L00315:75 ;
    skos:prefLabel "Item I84"@en-AU ;
    dcat:accessURL <https://www.legislation.gov.au/F2021L00315/2023-08-04/2023-08-04/text/original/epub/OEBPS/document_1/document_1.html#_Toc143853908> ;
    dcat:landingPage "https://www.legislation.gov.au/F2021L00315/2023-08-04/2023-08-04/text/original/epub/OEBPS/document_1/document_1.html#_Toc143853908"^^xsd:anyURI ;
    dcat:theme legcons:Item .

F2021L00315:85 a legcons:Item,
        owl:Class,
        dcat:Resource ;
    rdfs:label "Item - I85 4 11  Requirements for packages for export"@en-AU ;
    dct:isPartOf F2021L00315:75 ;
    dct:isReferencedBy F2021L00315: ;
    rdfs:comment "4 11  Requirements for packages for export - Abrievated Graph Key: I85"@en-AU ;
    skos:definition "4 11  Requirements for packages for export"@en-AU ;
    skos:narrower F2021L00315:75 ;
    skos:prefLabel "Item I85"@en-AU ;
    dcat:accessURL <https://www.legislation.gov.au/F2021L00315/2023-08-04/2023-08-04/text/original/epub/OEBPS/document_1/document_1.html#_Toc143853909> ;
    dcat:landingPage "https://www.legislation.gov.au/F2021L00315/2023-08-04/2023-08-04/text/original/epub/OEBPS/document_1/document_1.html#_Toc143853909"^^xsd:anyURI ;
    dcat:theme legcons:Item .

F2021L00315:86 a legcons:Item,
        owl:Class,
        dcat:Resource ;
    rdfs:label "Item - I86 4 12  Prescribed plants or plant products to be exported in bulk vessel"@en-AU ;
    dct:isPartOf F2021L00315:75 ;
    dct:isReferencedBy F2021L00315: ;
    rdfs:comment "4 12  Prescribed plants or plant products to be exported in bulk vessel - Abrievated Graph Key: I86"@en-AU ;
    skos:definition "4 12  Prescribed plants or plant products to be exported in bulk vessel"@en-AU ;
    skos:narrower F2021L00315:75 ;
    skos:prefLabel "Item I86"@en-AU ;
    dcat:accessURL <https://www.legislation.gov.au/F2021L00315/2023-08-04/2023-08-04/text/original/epub/OEBPS/document_1/document_1.html#_Toc143853910> ;
    dcat:landingPage "https://www.legislation.gov.au/F2021L00315/2023-08-04/2023-08-04/text/original/epub/OEBPS/document_1/document_1.html#_Toc143853910"^^xsd:anyURI ;
    dcat:theme legcons:Item .

F2021L00315:87 a legcons:Item,
        owl:Class,
        dcat:Resource ;
    rdfs:label "Item - I87 4 13  Prescribed plants or plant products to be exported in containers"@en-AU ;
    dct:isPartOf F2021L00315:75 ;
    dct:isReferencedBy F2021L00315: ;
    rdfs:comment "4 13  Prescribed plants or plant products to be exported in containers - Abrievated Graph Key: I87"@en-AU ;
    skos:definition "4 13  Prescribed plants or plant products to be exported in containers"@en-AU ;
    skos:narrower F2021L00315:75 ;
    skos:prefLabel "Item I87"@en-AU ;
    dcat:accessURL <https://www.legislation.gov.au/F2021L00315/2023-08-04/2023-08-04/text/original/epub/OEBPS/document_1/document_1.html#_Toc143853911> ;
    dcat:landingPage "https://www.legislation.gov.au/F2021L00315/2023-08-04/2023-08-04/text/original/epub/OEBPS/document_1/document_1.html#_Toc143853911"^^xsd:anyURI ;
    dcat:theme legcons:Item .

F2021L00315:89 a legcons:Item,
        owl:Class,
        dcat:Resource ;
    rdfs:label "Item - I89 4 14  Period within which application to renew registration must be made"@en-AU ;
    dct:isPartOf F2021L00315:88 ;
    dct:isReferencedBy F2021L00315: ;
    rdfs:comment "4 14  Period within which application to renew registration must be made - Abrievated Graph Key: I89"@en-AU ;
    skos:definition "4 14  Period within which application to renew registration must be made"@en-AU ;
    skos:narrower F2021L00315:88 ;
    skos:prefLabel "Item I89"@en-AU ;
    dcat:accessURL <https://www.legislation.gov.au/F2021L00315/2023-08-04/2023-08-04/text/original/epub/OEBPS/document_1/document_1.html#_Toc143853913> ;
    dcat:landingPage "https://www.legislation.gov.au/F2021L00315/2023-08-04/2023-08-04/text/original/epub/OEBPS/document_1/document_1.html#_Toc143853913"^^xsd:anyURI ;
    dcat:theme legcons:Item .

F2021L00315:9 a legcons:Item,
        owl:Class,
        dcat:Resource ;
    rdfs:label "Item - I9 1 7  Meaning of prescribed grain"@en-AU ;
    dct:isPartOf F2021L00315:1 ;
    dct:isReferencedBy F2021L00315: ;
    rdfs:comment "1 7  Meaning of prescribed grain - Abrievated Graph Key: I9"@en-AU ;
    skos:definition "1 7  Meaning of prescribed grain"@en-AU ;
    skos:narrower F2021L00315:1 ;
    skos:prefLabel "Item I9"@en-AU ;
    dcat:accessURL <https://www.legislation.gov.au/F2021L00315/2023-08-04/2023-08-04/text/original/epub/OEBPS/document_1/document_1.html#_Toc143853833> ;
    dcat:landingPage "https://www.legislation.gov.au/F2021L00315/2023-08-04/2023-08-04/text/original/epub/OEBPS/document_1/document_1.html#_Toc143853833"^^xsd:anyURI ;
    dcat:theme legcons:Item .

F2021L00315:90 a legcons:Item,
        owl:Class,
        dcat:Resource ;
    rdfs:label "Item - I90 4 15  Requirements for renewal of registration"@en-AU ;
    dct:isPartOf F2021L00315:88 ;
    dct:isReferencedBy F2021L00315: ;
    rdfs:comment "4 15  Requirements for renewal of registration - Abrievated Graph Key: I90"@en-AU ;
    skos:definition "4 15  Requirements for renewal of registration"@en-AU ;
    skos:narrower F2021L00315:88 ;
    skos:prefLabel "Item I90"@en-AU ;
    dcat:accessURL <https://www.legislation.gov.au/F2021L00315/2023-08-04/2023-08-04/text/original/epub/OEBPS/document_1/document_1.html#_Toc143853914> ;
    dcat:landingPage "https://www.legislation.gov.au/F2021L00315/2023-08-04/2023-08-04/text/original/epub/OEBPS/document_1/document_1.html#_Toc143853914"^^xsd:anyURI ;
    dcat:theme legcons:Item .

F2021L00315:92 a legcons:Item,
        owl:Class,
        dcat:Resource ;
    rdfs:label "Item - I92 4 16  Alterations for which approval is not required"@en-AU ;
    dct:isPartOf F2021L00315:91 ;
    dct:isReferencedBy F2021L00315: ;
    rdfs:comment "4 16  Alterations for which approval is not required - Abrievated Graph Key: I92"@en-AU ;
    skos:definition "4 16  Alterations for which approval is not required"@en-AU ;
    skos:narrower F2021L00315:91 ;
    skos:prefLabel "Item I92"@en-AU ;
    dcat:accessURL <https://www.legislation.gov.au/F2021L00315/2023-08-04/2023-08-04/text/original/epub/OEBPS/document_1/document_1.html#_Toc143853916> ;
    dcat:landingPage "https://www.legislation.gov.au/F2021L00315/2023-08-04/2023-08-04/text/original/epub/OEBPS/document_1/document_1.html#_Toc143853916"^^xsd:anyURI ;
    dcat:theme legcons:Item .

F2021L00315:93 a legcons:Item,
        owl:Class,
        dcat:Resource ;
    rdfs:label "Item - I93 4 17  Other reasons for the Secretary to vary registration"@en-AU ;
    dct:isPartOf F2021L00315:91 ;
    dct:isReferencedBy F2021L00315: ;
    rdfs:comment "4 17  Other reasons for the Secretary to vary registration - Abrievated Graph Key: I93"@en-AU ;
    skos:definition "4 17  Other reasons for the Secretary to vary registration"@en-AU ;
    skos:narrower F2021L00315:91 ;
    skos:prefLabel "Item I93"@en-AU ;
    dcat:accessURL <https://www.legislation.gov.au/F2021L00315/2023-08-04/2023-08-04/text/original/epub/OEBPS/document_1/document_1.html#_Toc143853917> ;
    dcat:landingPage "https://www.legislation.gov.au/F2021L00315/2023-08-04/2023-08-04/text/original/epub/OEBPS/document_1/document_1.html#_Toc143853917"^^xsd:anyURI ;
    dcat:theme legcons:Item .

F2021L00315:96 a legcons:Item,
        owl:Class,
        dcat:Resource ;
    rdfs:label "Item - I96 4 18  Circumstances in which occupier may request suspension of registration"@en-AU ;
    dct:isPartOf F2021L00315:95 ;
    dct:isReferencedBy F2021L00315: ;
    rdfs:comment "4 18  Circumstances in which occupier may request suspension of registration - Abrievated Graph Key: I96"@en-AU ;
    skos:definition "4 18  Circumstances in which occupier may request suspension of registration"@en-AU ;
    skos:narrower F2021L00315:95 ;
    skos:prefLabel "Item I96"@en-AU ;
    dcat:accessURL <https://www.legislation.gov.au/F2021L00315/2023-08-04/2023-08-04/text/original/epub/OEBPS/document_1/document_1.html#_Toc143853920> ;
    dcat:landingPage "https://www.legislation.gov.au/F2021L00315/2023-08-04/2023-08-04/text/original/epub/OEBPS/document_1/document_1.html#_Toc143853920"^^xsd:anyURI ;
    dcat:theme legcons:Item .

F2021L00315:98 a legcons:Item,
        owl:Class,
        dcat:Resource ;
    rdfs:label "Item - I98 4 19  Other grounds for suspension of registration"@en-AU ;
    dct:isPartOf F2021L00315:97 ;
    dct:isReferencedBy F2021L00315: ;
    rdfs:comment "4 19  Other grounds for suspension of registration - Abrievated Graph Key: I98"@en-AU ;
    skos:definition "4 19  Other grounds for suspension of registration"@en-AU ;
    skos:narrower F2021L00315:97 ;
    skos:prefLabel "Item I98"@en-AU ;
    dcat:accessURL <https://www.legislation.gov.au/F2021L00315/2023-08-04/2023-08-04/text/original/epub/OEBPS/document_1/document_1.html#_Toc143853922> ;
    dcat:landingPage "https://www.legislation.gov.au/F2021L00315/2023-08-04/2023-08-04/text/original/epub/OEBPS/document_1/document_1.html#_Toc143853922"^^xsd:anyURI ;
    dcat:theme legcons:Item .

F2021L00315:100 a legcons:Division,
        owl:Class,
        dcat:Resource ;
    rdfs:label "Division - D100 Division 1 Revocation requested by occupier"@en-AU ;
    dct:hasPart F2021L00315:101 ;
    dct:isPartOf F2021L00315:99 ;
    dct:isReferencedBy F2021L00315: ;
    rdfs:comment "Division 1 Revocation requested by occupier - Abrievated Graph Key: D100"@en-AU ;
    skos:broader F2021L00315:101 ;
    skos:definition "Division 1 Revocation requested by occupier"@en-AU ;
    skos:narrower F2021L00315:99 ;
    skos:prefLabel "Division D100"@en-AU ;
    dcat:accessURL <https://www.legislation.gov.au/F2021L00315/2023-08-04/2023-08-04/text/original/epub/OEBPS/document_1/document_1.html#_Toc143853924> ;
    dcat:landingPage "https://www.legislation.gov.au/F2021L00315/2023-08-04/2023-08-04/text/original/epub/OEBPS/document_1/document_1.html#_Toc143853924"^^xsd:anyURI ;
    dcat:theme legcons:Division .

F2021L00315:102 a legcons:Division,
        owl:Class,
        dcat:Resource ;
    rdfs:label "Division - D102 Division 2 Revocation by Secretary"@en-AU ;
    dct:hasPart F2021L00315:103 ;
    dct:isPartOf F2021L00315:99 ;
    dct:isReferencedBy F2021L00315: ;
    rdfs:comment "Division 2 Revocation by Secretary - Abrievated Graph Key: D102"@en-AU ;
    skos:broader F2021L00315:103 ;
    skos:definition "Division 2 Revocation by Secretary"@en-AU ;
    skos:narrower F2021L00315:99 ;
    skos:prefLabel "Division D102"@en-AU ;
    dcat:accessURL <https://www.legislation.gov.au/F2021L00315/2023-08-04/2023-08-04/text/original/epub/OEBPS/document_1/document_1.html#_Toc143853926> ;
    dcat:landingPage "https://www.legislation.gov.au/F2021L00315/2023-08-04/2023-08-04/text/original/epub/OEBPS/document_1/document_1.html#_Toc143853926"^^xsd:anyURI ;
    dcat:theme legcons:Division .

F2021L00315:104 a legcons:Part,
        owl:Class,
        dcat:Resource ;
    rdfs:label "Part - P104 Part 7 Obligations of occupiers of registered establishments"@en-AU ;
    dct:hasPart F2021L00315:105 ;
    dct:isPartOf F2021L00315:70 ;
    dct:isReferencedBy F2021L00315: ;
    rdfs:comment "Part 7 Obligations of occupiers of registered establishments - Abrievated Graph Key: P104"@en-AU ;
    skos:broader F2021L00315:105 ;
    skos:definition "Part 7 Obligations of occupiers of registered establishments"@en-AU ;
    skos:narrower F2021L00315:70 ;
    skos:prefLabel "Part P104"@en-AU ;
    dcat:accessURL <https://www.legislation.gov.au/F2021L00315/2023-08-04/2023-08-04/text/original/epub/OEBPS/document_1/document_1.html#_Toc143853928> ;
    dcat:landingPage "https://www.legislation.gov.au/F2021L00315/2023-08-04/2023-08-04/text/original/epub/OEBPS/document_1/document_1.html#_Toc143853928"^^xsd:anyURI ;
    dcat:theme legcons:Part .

F2021L00315:216 a legcons:Chapter,
        owl:Class,
        dcat:Resource ;
    rdfs:label "Chapter - C216 Chapter 10 Compliance and enforcement"@en-AU ;
    dct:hasPart F2021L00315:217,
        F2021L00315:218 ;
    dct:isReferencedBy F2021L00315: ;
    rdfs:comment "Chapter 10 Compliance and enforcement - Abrievated Graph Key: C216"@en-AU ;
    skos:broader F2021L00315:217,
        F2021L00315:218 ;
    skos:definition "Chapter 10 Compliance and enforcement"@en-AU ;
    skos:prefLabel "Chapter C216"@en-AU ;
    dcat:accessURL <https://www.legislation.gov.au/F2021L00315/2023-08-04/2023-08-04/text/original/epub/OEBPS/document_1/document_1.html#_Toc143854040> ;
    dcat:landingPage "https://www.legislation.gov.au/F2021L00315/2023-08-04/2023-08-04/text/original/epub/OEBPS/document_1/document_1.html#_Toc143854040"^^xsd:anyURI ;
    dcat:theme legcons:Chapter .

F2021L00315:232 a legcons:Part,
        owl:Class,
        dcat:Resource ;
    rdfs:label "Part - P232 Part 2 Samples"@en-AU ;
    dct:hasPart F2021L00315:233 ;
    dct:isPartOf F2021L00315:219 ;
    dct:isReferencedBy F2021L00315: ;
    rdfs:comment "Part 2 Samples - Abrievated Graph Key: P232"@en-AU ;
    skos:broader F2021L00315:233 ;
    skos:definition "Part 2 Samples"@en-AU ;
    skos:narrower F2021L00315:219 ;
    skos:prefLabel "Part P232"@en-AU ;
    dcat:accessURL <https://www.legislation.gov.au/F2021L00315/2023-08-04/2023-08-04/text/original/epub/OEBPS/document_1/document_1.html#_Toc143854056> ;
    dcat:landingPage "https://www.legislation.gov.au/F2021L00315/2023-08-04/2023-08-04/text/original/epub/OEBPS/document_1/document_1.html#_Toc143854056"^^xsd:anyURI ;
    dcat:theme legcons:Part .

F2021L00315:237 a legcons:Part,
        owl:Class,
        dcat:Resource ;
    rdfs:label "Part - P237 Part 4 Relevant Commonwealth liabilities"@en-AU ;
    dct:hasPart F2021L00315:238 ;
    dct:isPartOf F2021L00315:219 ;
    dct:isReferencedBy F2021L00315: ;
    rdfs:comment "Part 4 Relevant Commonwealth liabilities - Abrievated Graph Key: P237"@en-AU ;
    skos:broader F2021L00315:238 ;
    skos:definition "Part 4 Relevant Commonwealth liabilities"@en-AU ;
    skos:narrower F2021L00315:219 ;
    skos:prefLabel "Part P237"@en-AU ;
    dcat:accessURL <https://www.legislation.gov.au/F2021L00315/2023-08-04/2023-08-04/text/original/epub/OEBPS/document_1/document_1.html#_Toc143854061> ;
    dcat:landingPage "https://www.legislation.gov.au/F2021L00315/2023-08-04/2023-08-04/text/original/epub/OEBPS/document_1/document_1.html#_Toc143854061"^^xsd:anyURI ;
    dcat:theme legcons:Part .

F2021L00315:239 a legcons:Part,
        owl:Class,
        dcat:Resource ;
    rdfs:label "Part - P239 Part 5 Miscellaneous"@en-AU ;
    dct:hasPart F2021L00315:240 ;
    dct:isPartOf F2021L00315:219 ;
    dct:isReferencedBy F2021L00315: ;
    rdfs:comment "Part 5 Miscellaneous - Abrievated Graph Key: P239"@en-AU ;
    skos:broader F2021L00315:240 ;
    skos:definition "Part 5 Miscellaneous"@en-AU ;
    skos:narrower F2021L00315:219 ;
    skos:prefLabel "Part P239"@en-AU ;
    dcat:accessURL <https://www.legislation.gov.au/F2021L00315/2023-08-04/2023-08-04/text/original/epub/OEBPS/document_1/document_1.html#_Toc143854063> ;
    dcat:landingPage "https://www.legislation.gov.au/F2021L00315/2023-08-04/2023-08-04/text/original/epub/OEBPS/document_1/document_1.html#_Toc143854063"^^xsd:anyURI ;
    dcat:theme legcons:Part .

F2021L00315:242 a legcons:Part,
        owl:Class,
        dcat:Resource ;
    rdfs:label "Part - P242 Part 1 Preliminary"@en-AU ;
    dct:hasPart F2021L00315:243 ;
    dct:isPartOf F2021L00315:241 ;
    dct:isReferencedBy F2021L00315: ;
    rdfs:comment "Part 1 Preliminary - Abrievated Graph Key: P242"@en-AU ;
    skos:broader F2021L00315:243 ;
    skos:definition "Part 1 Preliminary"@en-AU ;
    skos:narrower F2021L00315:241 ;
    skos:prefLabel "Part P242"@en-AU ;
    dcat:accessURL <https://www.legislation.gov.au/F2021L00315/2023-08-04/2023-08-04/text/original/epub/OEBPS/document_1/document_1.html#_Toc143854066> ;
    dcat:landingPage "https://www.legislation.gov.au/F2021L00315/2023-08-04/2023-08-04/text/original/epub/OEBPS/document_1/document_1.html#_Toc143854066"^^xsd:anyURI ;
    dcat:theme legcons:Part .

F2021L00315:256 a legcons:Division,
        owl:Class,
        dcat:Resource ;
    rdfs:label "Division - D256 Division 1 Assessments"@en-AU ;
    dct:hasPart F2021L00315:257 ;
    dct:isPartOf F2021L00315:255 ;
    dct:isReferencedBy F2021L00315: ;
    rdfs:comment "Division 1 Assessments - Abrievated Graph Key: D256"@en-AU ;
    skos:broader F2021L00315:257 ;
    skos:definition "Division 1 Assessments"@en-AU ;
    skos:narrower F2021L00315:255 ;
    skos:prefLabel "Division D256"@en-AU ;
    dcat:accessURL <https://www.legislation.gov.au/F2021L00315/2023-08-04/2023-08-04/text/original/epub/OEBPS/document_1/document_1.html#_Toc143854080> ;
    dcat:landingPage "https://www.legislation.gov.au/F2021L00315/2023-08-04/2023-08-04/text/original/epub/OEBPS/document_1/document_1.html#_Toc143854080"^^xsd:anyURI ;
    dcat:theme legcons:Division .

F2021L00315:262 a legcons:Division,
        owl:Class,
        dcat:Resource ;
    rdfs:label "Division - D262 Division 3 Container approvals"@en-AU ;
    dct:hasPart F2021L00315:263 ;
    dct:isPartOf F2021L00315:255 ;
    dct:isReferencedBy F2021L00315: ;
    rdfs:comment "Division 3 Container approvals - Abrievated Graph Key: D262"@en-AU ;
    skos:broader F2021L00315:263 ;
    skos:definition "Division 3 Container approvals"@en-AU ;
    skos:narrower F2021L00315:255 ;
    skos:prefLabel "Division D262"@en-AU ;
    dcat:accessURL <https://www.legislation.gov.au/F2021L00315/2023-08-04/2023-08-04/text/original/epub/OEBPS/document_1/document_1.html#_Toc143854086> ;
    dcat:landingPage "https://www.legislation.gov.au/F2021L00315/2023-08-04/2023-08-04/text/original/epub/OEBPS/document_1/document_1.html#_Toc143854086"^^xsd:anyURI ;
    dcat:theme legcons:Division .

F2021L00315:35 a legcons:Division,
        owl:Class,
        dcat:Resource ;
    rdfs:label "Division - D35 Division 4 Other matters"@en-AU ;
    dct:hasPart F2021L00315:36 ;
    dct:isPartOf F2021L00315:11 ;
    dct:isReferencedBy F2021L00315: ;
    rdfs:comment "Division 4 Other matters - Abrievated Graph Key: D35"@en-AU ;
    skos:broader F2021L00315:36 ;
    skos:definition "Division 4 Other matters"@en-AU ;
    skos:narrower F2021L00315:11 ;
    skos:prefLabel "Division D35"@en-AU ;
    dcat:accessURL <https://www.legislation.gov.au/F2021L00315/2023-08-04/2023-08-04/text/original/epub/OEBPS/document_1/document_1.html#_Toc143853859> ;
    dcat:landingPage "https://www.legislation.gov.au/F2021L00315/2023-08-04/2023-08-04/text/original/epub/OEBPS/document_1/document_1.html#_Toc143853859"^^xsd:anyURI ;
    dcat:theme legcons:Division .

F2021L00315:38 a legcons:Part,
        owl:Class,
        dcat:Resource ;
    rdfs:label "Part - P38 Part 1 Requirements for accreditation"@en-AU ;
    dct:hasPart F2021L00315:39 ;
    dct:isPartOf F2021L00315:37 ;
    dct:isReferencedBy F2021L00315: ;
    rdfs:comment "Part 1 Requirements for accreditation - Abrievated Graph Key: P38"@en-AU ;
    skos:broader F2021L00315:39 ;
    skos:definition "Part 1 Requirements for accreditation"@en-AU ;
    skos:narrower F2021L00315:37 ;
    skos:prefLabel "Part P38"@en-AU ;
    dcat:accessURL <https://www.legislation.gov.au/F2021L00315/2023-08-04/2023-08-04/text/original/epub/OEBPS/document_1/document_1.html#_Toc143853862> ;
    dcat:landingPage "https://www.legislation.gov.au/F2021L00315/2023-08-04/2023-08-04/text/original/epub/OEBPS/document_1/document_1.html#_Toc143853862"^^xsd:anyURI ;
    dcat:theme legcons:Part .

F2021L00315:55 a legcons:Division,
        owl:Class,
        dcat:Resource ;
    rdfs:label "Division - D55 Division 1 Suspension requested by manager"@en-AU ;
    dct:hasPart F2021L00315:56 ;
    dct:isPartOf F2021L00315:54 ;
    dct:isReferencedBy F2021L00315: ;
    rdfs:comment "Division 1 Suspension requested by manager - Abrievated Graph Key: D55"@en-AU ;
    skos:broader F2021L00315:56 ;
    skos:definition "Division 1 Suspension requested by manager"@en-AU ;
    skos:narrower F2021L00315:54 ;
    skos:prefLabel "Division D55"@en-AU ;
    dcat:accessURL <https://www.legislation.gov.au/F2021L00315/2023-08-04/2023-08-04/text/original/epub/OEBPS/document_1/document_1.html#_Toc143853879> ;
    dcat:landingPage "https://www.legislation.gov.au/F2021L00315/2023-08-04/2023-08-04/text/original/epub/OEBPS/document_1/document_1.html#_Toc143853879"^^xsd:anyURI ;
    dcat:theme legcons:Division .

F2021L00315:57 a legcons:Division,
        owl:Class,
        dcat:Resource ;
    rdfs:label "Division - D57 Division 2 Suspension by Secretary"@en-AU ;
    dct:hasPart F2021L00315:58 ;
    dct:isPartOf F2021L00315:54 ;
    dct:isReferencedBy F2021L00315: ;
    rdfs:comment "Division 2 Suspension by Secretary - Abrievated Graph Key: D57"@en-AU ;
    skos:broader F2021L00315:58 ;
    skos:definition "Division 2 Suspension by Secretary"@en-AU ;
    skos:narrower F2021L00315:54 ;
    skos:prefLabel "Division D57"@en-AU ;
    dcat:accessURL <https://www.legislation.gov.au/F2021L00315/2023-08-04/2023-08-04/text/original/epub/OEBPS/document_1/document_1.html#_Toc143853881> ;
    dcat:landingPage "https://www.legislation.gov.au/F2021L00315/2023-08-04/2023-08-04/text/original/epub/OEBPS/document_1/document_1.html#_Toc143853881"^^xsd:anyURI ;
    dcat:theme legcons:Division .

F2021L00315:60 a legcons:Division,
        owl:Class,
        dcat:Resource ;
    rdfs:label "Division - D60 Division 1 Revocation requested by manager"@en-AU ;
    dct:hasPart F2021L00315:61 ;
    dct:isPartOf F2021L00315:59 ;
    dct:isReferencedBy F2021L00315: ;
    rdfs:comment "Division 1 Revocation requested by manager - Abrievated Graph Key: D60"@en-AU ;
    skos:broader F2021L00315:61 ;
    skos:definition "Division 1 Revocation requested by manager"@en-AU ;
    skos:narrower F2021L00315:59 ;
    skos:prefLabel "Division D60"@en-AU ;
    dcat:accessURL <https://www.legislation.gov.au/F2021L00315/2023-08-04/2023-08-04/text/original/epub/OEBPS/document_1/document_1.html#_Toc143853884> ;
    dcat:landingPage "https://www.legislation.gov.au/F2021L00315/2023-08-04/2023-08-04/text/original/epub/OEBPS/document_1/document_1.html#_Toc143853884"^^xsd:anyURI ;
    dcat:theme legcons:Division .

F2021L00315:62 a legcons:Division,
        owl:Class,
        dcat:Resource ;
    rdfs:label "Division - D62 Division 2 Revocation by Secretary"@en-AU ;
    dct:hasPart F2021L00315:63 ;
    dct:isPartOf F2021L00315:59 ;
    dct:isReferencedBy F2021L00315: ;
    rdfs:comment "Division 2 Revocation by Secretary - Abrievated Graph Key: D62"@en-AU ;
    skos:broader F2021L00315:63 ;
    skos:definition "Division 2 Revocation by Secretary"@en-AU ;
    skos:narrower F2021L00315:59 ;
    skos:prefLabel "Division D62"@en-AU ;
    dcat:accessURL <https://www.legislation.gov.au/F2021L00315/2023-08-04/2023-08-04/text/original/epub/OEBPS/document_1/document_1.html#_Toc143853886> ;
    dcat:landingPage "https://www.legislation.gov.au/F2021L00315/2023-08-04/2023-08-04/text/original/epub/OEBPS/document_1/document_1.html#_Toc143853886"^^xsd:anyURI ;
    dcat:theme legcons:Division .

F2021L00315:64 a legcons:Part,
        owl:Class,
        dcat:Resource ;
    rdfs:label "Part - P64 Part 7 Obligations of managers of accredited properties etc"@en-AU ;
    dct:hasPart F2021L00315:65 ;
    dct:isPartOf F2021L00315:37 ;
    dct:isReferencedBy F2021L00315: ;
    rdfs:comment "Part 7 Obligations of managers of accredited properties etc - Abrievated Graph Key: P64"@en-AU ;
    skos:broader F2021L00315:65 ;
    skos:definition "Part 7 Obligations of managers of accredited properties etc"@en-AU ;
    skos:narrower F2021L00315:37 ;
    skos:prefLabel "Part P64"@en-AU ;
    dcat:accessURL <https://www.legislation.gov.au/F2021L00315/2023-08-04/2023-08-04/text/original/epub/OEBPS/document_1/document_1.html#_Toc143853888> ;
    dcat:landingPage "https://www.legislation.gov.au/F2021L00315/2023-08-04/2023-08-04/text/original/epub/OEBPS/document_1/document_1.html#_Toc143853888"^^xsd:anyURI ;
    dcat:theme legcons:Part .

F2021L00315:95 a legcons:Division,
        owl:Class,
        dcat:Resource ;
    rdfs:label "Division - D95 Division 1 Suspension requested by occupier"@en-AU ;
    dct:hasPart F2021L00315:96 ;
    dct:isPartOf F2021L00315:94 ;
    dct:isReferencedBy F2021L00315: ;
    rdfs:comment "Division 1 Suspension requested by occupier - Abrievated Graph Key: D95"@en-AU ;
    skos:broader F2021L00315:96 ;
    skos:definition "Division 1 Suspension requested by occupier"@en-AU ;
    skos:narrower F2021L00315:94 ;
    skos:prefLabel "Division D95"@en-AU ;
    dcat:accessURL <https://www.legislation.gov.au/F2021L00315/2023-08-04/2023-08-04/text/original/epub/OEBPS/document_1/document_1.html#_Toc143853919> ;
    dcat:landingPage "https://www.legislation.gov.au/F2021L00315/2023-08-04/2023-08-04/text/original/epub/OEBPS/document_1/document_1.html#_Toc143853919"^^xsd:anyURI ;
    dcat:theme legcons:Division .

F2021L00315:97 a legcons:Division,
        owl:Class,
        dcat:Resource ;
    rdfs:label "Division - D97 Division 2 Suspension by Secretary"@en-AU ;
    dct:hasPart F2021L00315:98 ;
    dct:isPartOf F2021L00315:94 ;
    dct:isReferencedBy F2021L00315: ;
    rdfs:comment "Division 2 Suspension by Secretary - Abrievated Graph Key: D97"@en-AU ;
    skos:broader F2021L00315:98 ;
    skos:definition "Division 2 Suspension by Secretary"@en-AU ;
    skos:narrower F2021L00315:94 ;
    skos:prefLabel "Division D97"@en-AU ;
    dcat:accessURL <https://www.legislation.gov.au/F2021L00315/2023-08-04/2023-08-04/text/original/epub/OEBPS/document_1/document_1.html#_Toc143853921> ;
    dcat:landingPage "https://www.legislation.gov.au/F2021L00315/2023-08-04/2023-08-04/text/original/epub/OEBPS/document_1/document_1.html#_Toc143853921"^^xsd:anyURI ;
    dcat:theme legcons:Division .

F2021L00315:111 a legcons:Part,
        owl:Class,
        dcat:Resource ;
    rdfs:label "Part - P111 Part 1 Issue of export permit"@en-AU ;
    dct:hasPart F2021L00315:112,
        F2021L00315:113 ;
    dct:isPartOf F2021L00315:110 ;
    dct:isReferencedBy F2021L00315: ;
    rdfs:comment "Part 1 Issue of export permit - Abrievated Graph Key: P111"@en-AU ;
    skos:broader F2021L00315:112,
        F2021L00315:113 ;
    skos:definition "Part 1 Issue of export permit"@en-AU ;
    skos:narrower F2021L00315:110 ;
    skos:prefLabel "Part P111"@en-AU ;
    dcat:accessURL <https://www.legislation.gov.au/F2021L00315/2023-08-04/2023-08-04/text/original/epub/OEBPS/document_1/document_1.html#_Toc143853935> ;
    dcat:landingPage "https://www.legislation.gov.au/F2021L00315/2023-08-04/2023-08-04/text/original/epub/OEBPS/document_1/document_1.html#_Toc143853935"^^xsd:anyURI ;
    dcat:theme legcons:Part .

F2021L00315:119 a legcons:Part,
        owl:Class,
        dcat:Resource ;
    rdfs:label "Part - P119 Part 3 Other matters"@en-AU ;
    dct:hasPart F2021L00315:120,
        F2021L00315:121 ;
    dct:isPartOf F2021L00315:110 ;
    dct:isReferencedBy F2021L00315: ;
    rdfs:comment "Part 3 Other matters - Abrievated Graph Key: P119"@en-AU ;
    skos:broader F2021L00315:120,
        F2021L00315:121 ;
    skos:definition "Part 3 Other matters"@en-AU ;
    skos:narrower F2021L00315:110 ;
    skos:prefLabel "Part P119"@en-AU ;
    dcat:accessURL <https://www.legislation.gov.au/F2021L00315/2023-08-04/2023-08-04/text/original/epub/OEBPS/document_1/document_1.html#_Toc143853943> ;
    dcat:landingPage "https://www.legislation.gov.au/F2021L00315/2023-08-04/2023-08-04/text/original/epub/OEBPS/document_1/document_1.html#_Toc143853943"^^xsd:anyURI ;
    dcat:theme legcons:Part .

F2021L00315:122 a legcons:Part,
        owl:Class,
        dcat:Resource ;
    rdfs:label "Part - P122 Part 4 Applications for export permits"@en-AU ;
    dct:hasPart F2021L00315:123,
        F2021L00315:124 ;
    dct:isPartOf F2021L00315:110 ;
    dct:isReferencedBy F2021L00315: ;
    rdfs:comment "Part 4 Applications for export permits - Abrievated Graph Key: P122"@en-AU ;
    skos:broader F2021L00315:123,
        F2021L00315:124 ;
    skos:definition "Part 4 Applications for export permits"@en-AU ;
    skos:narrower F2021L00315:110 ;
    skos:prefLabel "Part P122"@en-AU ;
    dcat:accessURL <https://www.legislation.gov.au/F2021L00315/2023-08-04/2023-08-04/text/original/epub/OEBPS/document_1/document_1.html#_Toc143853946> ;
    dcat:landingPage "https://www.legislation.gov.au/F2021L00315/2023-08-04/2023-08-04/text/original/epub/OEBPS/document_1/document_1.html#_Toc143853946"^^xsd:anyURI ;
    dcat:theme legcons:Part .

F2021L00315:125 a legcons:Chapter,
        owl:Class,
        dcat:Resource ;
    rdfs:label "Chapter - C125 Chapter 8 Other matters relating to export"@en-AU ;
    dct:hasPart F2021L00315:126,
        F2021L00315:131,
        F2021L00315:136 ;
    dct:isReferencedBy F2021L00315: ;
    rdfs:comment "Chapter 8 Other matters relating to export - Abrievated Graph Key: C125"@en-AU ;
    skos:broader F2021L00315:126,
        F2021L00315:131,
        F2021L00315:136 ;
    skos:definition "Chapter 8 Other matters relating to export"@en-AU ;
    skos:prefLabel "Chapter C125"@en-AU ;
    dcat:accessURL <https://www.legislation.gov.au/F2021L00315/2023-08-04/2023-08-04/text/original/epub/OEBPS/document_1/document_1.html#_Toc143853949> ;
    dcat:landingPage "https://www.legislation.gov.au/F2021L00315/2023-08-04/2023-08-04/text/original/epub/OEBPS/document_1/document_1.html#_Toc143853949"^^xsd:anyURI ;
    dcat:theme legcons:Chapter .

F2021L00315:13 a legcons:Division,
        owl:Class,
        dcat:Resource ;
    rdfs:label "Division - D13 Division 1 Prescribed goods"@en-AU ;
    dct:hasPart F2021L00315:14,
        F2021L00315:15 ;
    dct:isPartOf F2021L00315:12 ;
    dct:isReferencedBy F2021L00315: ;
    rdfs:comment "Division 1 Prescribed goods - Abrievated Graph Key: D13"@en-AU ;
    skos:broader F2021L00315:14,
        F2021L00315:15 ;
    skos:definition "Division 1 Prescribed goods"@en-AU ;
    skos:narrower F2021L00315:12 ;
    skos:prefLabel "Division D13"@en-AU ;
    dcat:accessURL <https://www.legislation.gov.au/F2021L00315/2023-08-04/2023-08-04/text/original/epub/OEBPS/document_1/document_1.html#_Toc143853837> ;
    dcat:landingPage "https://www.legislation.gov.au/F2021L00315/2023-08-04/2023-08-04/text/original/epub/OEBPS/document_1/document_1.html#_Toc143853837"^^xsd:anyURI ;
    dcat:theme legcons:Division .

F2021L00315:169 a legcons:Part,
        owl:Class,
        dcat:Resource ;
    rdfs:label "Part - P169 Part 1 Audits"@en-AU ;
    dct:hasPart F2021L00315:170,
        F2021L00315:173 ;
    dct:isPartOf F2021L00315:168 ;
    dct:isReferencedBy F2021L00315: ;
    rdfs:comment "Part 1 Audits - Abrievated Graph Key: P169"@en-AU ;
    skos:broader F2021L00315:170,
        F2021L00315:173 ;
    skos:definition "Part 1 Audits"@en-AU ;
    skos:narrower F2021L00315:168 ;
    skos:prefLabel "Part P169"@en-AU ;
    dcat:accessURL <https://www.legislation.gov.au/F2021L00315/2023-08-04/2023-08-04/text/original/epub/OEBPS/document_1/document_1.html#_Toc143853993> ;
    dcat:landingPage "https://www.legislation.gov.au/F2021L00315/2023-08-04/2023-08-04/text/original/epub/OEBPS/document_1/document_1.html#_Toc143853993"^^xsd:anyURI ;
    dcat:theme legcons:Part .

F2021L00315:170 a legcons:Division,
        owl:Class,
        dcat:Resource ;
    rdfs:label "Division - D170 Division 1 General"@en-AU ;
    dct:hasPart F2021L00315:171,
        F2021L00315:172 ;
    dct:isPartOf F2021L00315:169 ;
    dct:isReferencedBy F2021L00315: ;
    rdfs:comment "Division 1 General - Abrievated Graph Key: D170"@en-AU ;
    skos:broader F2021L00315:171,
        F2021L00315:172 ;
    skos:definition "Division 1 General"@en-AU ;
    skos:narrower F2021L00315:169 ;
    skos:prefLabel "Division D170"@en-AU ;
    dcat:accessURL <https://www.legislation.gov.au/F2021L00315/2023-08-04/2023-08-04/text/original/epub/OEBPS/document_1/document_1.html#_Toc143853994> ;
    dcat:landingPage "https://www.legislation.gov.au/F2021L00315/2023-08-04/2023-08-04/text/original/epub/OEBPS/document_1/document_1.html#_Toc143853994"^^xsd:anyURI ;
    dcat:theme legcons:Division .

F2021L00315:173 a legcons:Division,
        owl:Class,
        dcat:Resource ;
    rdfs:label "Division - D173 Division 2 Conduct of audit etc"@en-AU ;
    dct:hasPart F2021L00315:174,
        F2021L00315:175 ;
    dct:isPartOf F2021L00315:169 ;
    dct:isReferencedBy F2021L00315: ;
    rdfs:comment "Division 2 Conduct of audit etc - Abrievated Graph Key: D173"@en-AU ;
    skos:broader F2021L00315:174,
        F2021L00315:175 ;
    skos:definition "Division 2 Conduct of audit etc"@en-AU ;
    skos:narrower F2021L00315:169 ;
    skos:prefLabel "Division D173"@en-AU ;
    dcat:accessURL <https://www.legislation.gov.au/F2021L00315/2023-08-04/2023-08-04/text/original/epub/OEBPS/document_1/document_1.html#_Toc143853997> ;
    dcat:landingPage "https://www.legislation.gov.au/F2021L00315/2023-08-04/2023-08-04/text/original/epub/OEBPS/document_1/document_1.html#_Toc143853997"^^xsd:anyURI ;
    dcat:theme legcons:Division .

F2021L00315:176 a legcons:Part,
        owl:Class,
        dcat:Resource ;
    rdfs:label "Part - P176 Part 2 Assessments"@en-AU ;
    dct:hasPart F2021L00315:177,
        F2021L00315:180 ;
    dct:isPartOf F2021L00315:168 ;
    dct:isReferencedBy F2021L00315: ;
    rdfs:comment "Part 2 Assessments - Abrievated Graph Key: P176"@en-AU ;
    skos:broader F2021L00315:177,
        F2021L00315:180 ;
    skos:definition "Part 2 Assessments"@en-AU ;
    skos:narrower F2021L00315:168 ;
    skos:prefLabel "Part P176"@en-AU ;
    dcat:accessURL <https://www.legislation.gov.au/F2021L00315/2023-08-04/2023-08-04/text/original/epub/OEBPS/document_1/document_1.html#_Toc143854000> ;
    dcat:landingPage "https://www.legislation.gov.au/F2021L00315/2023-08-04/2023-08-04/text/original/epub/OEBPS/document_1/document_1.html#_Toc143854000"^^xsd:anyURI ;
    dcat:theme legcons:Part .

F2021L00315:177 a legcons:Division,
        owl:Class,
        dcat:Resource ;
    rdfs:label "Division - D177 Division 1 General"@en-AU ;
    dct:hasPart F2021L00315:178,
        F2021L00315:179 ;
    dct:isPartOf F2021L00315:176 ;
    dct:isReferencedBy F2021L00315: ;
    rdfs:comment "Division 1 General - Abrievated Graph Key: D177"@en-AU ;
    skos:broader F2021L00315:178,
        F2021L00315:179 ;
    skos:definition "Division 1 General"@en-AU ;
    skos:narrower F2021L00315:176 ;
    skos:prefLabel "Division D177"@en-AU ;
    dcat:accessURL <https://www.legislation.gov.au/F2021L00315/2023-08-04/2023-08-04/text/original/epub/OEBPS/document_1/document_1.html#_Toc143854001> ;
    dcat:landingPage "https://www.legislation.gov.au/F2021L00315/2023-08-04/2023-08-04/text/original/epub/OEBPS/document_1/document_1.html#_Toc143854001"^^xsd:anyURI ;
    dcat:theme legcons:Division .

F2021L00315:191 a legcons:Part,
        owl:Class,
        dcat:Resource ;
    rdfs:label "Part - P191 Part 3 Powers of the Secretary"@en-AU ;
    dct:hasPart F2021L00315:192,
        F2021L00315:193 ;
    dct:isPartOf F2021L00315:168 ;
    dct:isReferencedBy F2021L00315: ;
    rdfs:comment "Part 3 Powers of the Secretary - Abrievated Graph Key: P191"@en-AU ;
    skos:broader F2021L00315:192,
        F2021L00315:193 ;
    skos:definition "Part 3 Powers of the Secretary"@en-AU ;
    skos:narrower F2021L00315:168 ;
    skos:prefLabel "Part P191"@en-AU ;
    dcat:accessURL <https://www.legislation.gov.au/F2021L00315/2023-08-04/2023-08-04/text/original/epub/OEBPS/document_1/document_1.html#_Toc143854015> ;
    dcat:landingPage "https://www.legislation.gov.au/F2021L00315/2023-08-04/2023-08-04/text/original/epub/OEBPS/document_1/document_1.html#_Toc143854015"^^xsd:anyURI ;
    dcat:theme legcons:Part .

F2021L00315:234 a legcons:Part,
        owl:Class,
        dcat:Resource ;
    rdfs:label "Part - P234 Part 3 Damaged or destroyed plants or plant products"@en-AU ;
    dct:hasPart F2021L00315:235,
        F2021L00315:236 ;
    dct:isPartOf F2021L00315:219 ;
    dct:isReferencedBy F2021L00315: ;
    rdfs:comment "Part 3 Damaged or destroyed plants or plant products - Abrievated Graph Key: P234"@en-AU ;
    skos:broader F2021L00315:235,
        F2021L00315:236 ;
    skos:definition "Part 3 Damaged or destroyed plants or plant products"@en-AU ;
    skos:narrower F2021L00315:219 ;
    skos:prefLabel "Part P234"@en-AU ;
    dcat:accessURL <https://www.legislation.gov.au/F2021L00315/2023-08-04/2023-08-04/text/original/epub/OEBPS/document_1/document_1.html#_Toc143854058> ;
    dcat:landingPage "https://www.legislation.gov.au/F2021L00315/2023-08-04/2023-08-04/text/original/epub/OEBPS/document_1/document_1.html#_Toc143854058"^^xsd:anyURI ;
    dcat:theme legcons:Part .

F2021L00315:244 a legcons:Part,
        owl:Class,
        dcat:Resource ;
    rdfs:label "Part - P244 Part 2 Registered establishments"@en-AU ;
    dct:hasPart F2021L00315:245,
        F2021L00315:246 ;
    dct:isPartOf F2021L00315:241 ;
    dct:isReferencedBy F2021L00315: ;
    rdfs:comment "Part 2 Registered establishments - Abrievated Graph Key: P244"@en-AU ;
    skos:broader F2021L00315:245,
        F2021L00315:246 ;
    skos:definition "Part 2 Registered establishments"@en-AU ;
    skos:narrower F2021L00315:241 ;
    skos:prefLabel "Part P244"@en-AU ;
    dcat:accessURL <https://www.legislation.gov.au/F2021L00315/2023-08-04/2023-08-04/text/original/epub/OEBPS/document_1/document_1.html#_Toc143854068> ;
    dcat:landingPage "https://www.legislation.gov.au/F2021L00315/2023-08-04/2023-08-04/text/original/epub/OEBPS/document_1/document_1.html#_Toc143854068"^^xsd:anyURI ;
    dcat:theme legcons:Part .

F2021L00315:247 a legcons:Part,
        owl:Class,
        dcat:Resource ;
    rdfs:label "Part - P247 Part 3 Other matters relating to export"@en-AU ;
    dct:hasPart F2021L00315:248,
        F2021L00315:252 ;
    dct:isPartOf F2021L00315:241 ;
    dct:isReferencedBy F2021L00315: ;
    rdfs:comment "Part 3 Other matters relating to export - Abrievated Graph Key: P247"@en-AU ;
    skos:broader F2021L00315:248,
        F2021L00315:252 ;
    skos:definition "Part 3 Other matters relating to export"@en-AU ;
    skos:narrower F2021L00315:241 ;
    skos:prefLabel "Part P247"@en-AU ;
    dcat:accessURL <https://www.legislation.gov.au/F2021L00315/2023-08-04/2023-08-04/text/original/epub/OEBPS/document_1/document_1.html#_Toc143854071> ;
    dcat:landingPage "https://www.legislation.gov.au/F2021L00315/2023-08-04/2023-08-04/text/original/epub/OEBPS/document_1/document_1.html#_Toc143854071"^^xsd:anyURI ;
    dcat:theme legcons:Part .

F2021L00315:252 a legcons:Division,
        owl:Class,
        dcat:Resource ;
    rdfs:label "Division - D252 Division 2 Official marking devices"@en-AU ;
    dct:hasPart F2021L00315:253,
        F2021L00315:254 ;
    dct:isPartOf F2021L00315:247 ;
    dct:isReferencedBy F2021L00315: ;
    rdfs:comment "Division 2 Official marking devices - Abrievated Graph Key: D252"@en-AU ;
    skos:broader F2021L00315:253,
        F2021L00315:254 ;
    skos:definition "Division 2 Official marking devices"@en-AU ;
    skos:narrower F2021L00315:247 ;
    skos:prefLabel "Division D252"@en-AU ;
    dcat:accessURL <https://www.legislation.gov.au/F2021L00315/2023-08-04/2023-08-04/text/original/epub/OEBPS/document_1/document_1.html#_Toc143854076> ;
    dcat:landingPage "https://www.legislation.gov.au/F2021L00315/2023-08-04/2023-08-04/text/original/epub/OEBPS/document_1/document_1.html#_Toc143854076"^^xsd:anyURI ;
    dcat:theme legcons:Division .

F2021L00315:26 a legcons:Division,
        owl:Class,
        dcat:Resource ;
    rdfs:label "Division - D26 Division 1 General"@en-AU ;
    dct:hasPart F2021L00315:27,
        F2021L00315:28 ;
    dct:isPartOf F2021L00315:11 ;
    dct:isReferencedBy F2021L00315: ;
    rdfs:comment "Division 1 General - Abrievated Graph Key: D26"@en-AU ;
    skos:broader F2021L00315:27,
        F2021L00315:28 ;
    skos:definition "Division 1 General"@en-AU ;
    skos:narrower F2021L00315:11 ;
    skos:prefLabel "Division D26"@en-AU ;
    dcat:accessURL <https://www.legislation.gov.au/F2021L00315/2023-08-04/2023-08-04/text/original/epub/OEBPS/document_1/document_1.html#_Toc143853850> ;
    dcat:landingPage "https://www.legislation.gov.au/F2021L00315/2023-08-04/2023-08-04/text/original/epub/OEBPS/document_1/document_1.html#_Toc143853850"^^xsd:anyURI ;
    dcat:theme legcons:Division .

F2021L00315:29 a legcons:Division,
        owl:Class,
        dcat:Resource ;
    rdfs:label "Division - D29 Division 2 Phytosanitary certificates and phytosanitary certificates for re export"@en-AU ;
    dct:hasPart F2021L00315:30,
        F2021L00315:31 ;
    dct:isPartOf F2021L00315:11 ;
    dct:isReferencedBy F2021L00315: ;
    rdfs:comment "Division 2 Phytosanitary certificates and phytosanitary certificates for re export - Abrievated Graph Key: D29"@en-AU ;
    skos:broader F2021L00315:30,
        F2021L00315:31 ;
    skos:definition "Division 2 Phytosanitary certificates and phytosanitary certificates for re export"@en-AU ;
    skos:narrower F2021L00315:11 ;
    skos:prefLabel "Division D29"@en-AU ;
    dcat:accessURL <https://www.legislation.gov.au/F2021L00315/2023-08-04/2023-08-04/text/original/epub/OEBPS/document_1/document_1.html#_Toc143853853> ;
    dcat:landingPage "https://www.legislation.gov.au/F2021L00315/2023-08-04/2023-08-04/text/original/epub/OEBPS/document_1/document_1.html#_Toc143853853"^^xsd:anyURI ;
    dcat:theme legcons:Division .

F2021L00315:32 a legcons:Division,
        owl:Class,
        dcat:Resource ;
    rdfs:label "Division - D32 Division 3 Issue of government certificates"@en-AU ;
    dct:hasPart F2021L00315:33,
        F2021L00315:34 ;
    dct:isPartOf F2021L00315:11 ;
    dct:isReferencedBy F2021L00315: ;
    rdfs:comment "Division 3 Issue of government certificates - Abrievated Graph Key: D32"@en-AU ;
    skos:broader F2021L00315:33,
        F2021L00315:34 ;
    skos:definition "Division 3 Issue of government certificates"@en-AU ;
    skos:narrower F2021L00315:11 ;
    skos:prefLabel "Division D32"@en-AU ;
    dcat:accessURL <https://www.legislation.gov.au/F2021L00315/2023-08-04/2023-08-04/text/original/epub/OEBPS/document_1/document_1.html#_Toc143853856> ;
    dcat:landingPage "https://www.legislation.gov.au/F2021L00315/2023-08-04/2023-08-04/text/original/epub/OEBPS/document_1/document_1.html#_Toc143853856"^^xsd:anyURI ;
    dcat:theme legcons:Division .

F2021L00315:48 a legcons:Part,
        owl:Class,
        dcat:Resource ;
    rdfs:label "Part - P48 Part 3 Renewal of accreditation"@en-AU ;
    dct:hasPart F2021L00315:49,
        F2021L00315:50 ;
    dct:isPartOf F2021L00315:37 ;
    dct:isReferencedBy F2021L00315: ;
    rdfs:comment "Part 3 Renewal of accreditation - Abrievated Graph Key: P48"@en-AU ;
    skos:broader F2021L00315:49,
        F2021L00315:50 ;
    skos:definition "Part 3 Renewal of accreditation"@en-AU ;
    skos:narrower F2021L00315:37 ;
    skos:prefLabel "Part P48"@en-AU ;
    dcat:accessURL <https://www.legislation.gov.au/F2021L00315/2023-08-04/2023-08-04/text/original/epub/OEBPS/document_1/document_1.html#_Toc143853872> ;
    dcat:landingPage "https://www.legislation.gov.au/F2021L00315/2023-08-04/2023-08-04/text/original/epub/OEBPS/document_1/document_1.html#_Toc143853872"^^xsd:anyURI ;
    dcat:theme legcons:Part .

F2021L00315:51 a legcons:Part,
        owl:Class,
        dcat:Resource ;
    rdfs:label "Part - P51 Part 4 Variation of accreditation"@en-AU ;
    dct:hasPart F2021L00315:52,
        F2021L00315:53 ;
    dct:isPartOf F2021L00315:37 ;
    dct:isReferencedBy F2021L00315: ;
    rdfs:comment "Part 4 Variation of accreditation - Abrievated Graph Key: P51"@en-AU ;
    skos:broader F2021L00315:52,
        F2021L00315:53 ;
    skos:definition "Part 4 Variation of accreditation"@en-AU ;
    skos:narrower F2021L00315:37 ;
    skos:prefLabel "Part P51"@en-AU ;
    dcat:accessURL <https://www.legislation.gov.au/F2021L00315/2023-08-04/2023-08-04/text/original/epub/OEBPS/document_1/document_1.html#_Toc143853875> ;
    dcat:landingPage "https://www.legislation.gov.au/F2021L00315/2023-08-04/2023-08-04/text/original/epub/OEBPS/document_1/document_1.html#_Toc143853875"^^xsd:anyURI ;
    dcat:theme legcons:Part .

F2021L00315:54 a legcons:Part,
        owl:Class,
        dcat:Resource ;
    rdfs:label "Part - P54 Part 5 Suspension of accreditation"@en-AU ;
    dct:hasPart F2021L00315:55,
        F2021L00315:57 ;
    dct:isPartOf F2021L00315:37 ;
    dct:isReferencedBy F2021L00315: ;
    rdfs:comment "Part 5 Suspension of accreditation - Abrievated Graph Key: P54"@en-AU ;
    skos:broader F2021L00315:55,
        F2021L00315:57 ;
    skos:definition "Part 5 Suspension of accreditation"@en-AU ;
    skos:narrower F2021L00315:37 ;
    skos:prefLabel "Part P54"@en-AU ;
    dcat:accessURL <https://www.legislation.gov.au/F2021L00315/2023-08-04/2023-08-04/text/original/epub/OEBPS/document_1/document_1.html#_Toc143853878> ;
    dcat:landingPage "https://www.legislation.gov.au/F2021L00315/2023-08-04/2023-08-04/text/original/epub/OEBPS/document_1/document_1.html#_Toc143853878"^^xsd:anyURI ;
    dcat:theme legcons:Part .

F2021L00315:59 a legcons:Part,
        owl:Class,
        dcat:Resource ;
    rdfs:label "Part - P59 Part 6 Revocation of accreditation"@en-AU ;
    dct:hasPart F2021L00315:60,
        F2021L00315:62 ;
    dct:isPartOf F2021L00315:37 ;
    dct:isReferencedBy F2021L00315: ;
    rdfs:comment "Part 6 Revocation of accreditation - Abrievated Graph Key: P59"@en-AU ;
    skos:broader F2021L00315:60,
        F2021L00315:62 ;
    skos:definition "Part 6 Revocation of accreditation"@en-AU ;
    skos:narrower F2021L00315:37 ;
    skos:prefLabel "Part P59"@en-AU ;
    dcat:accessURL <https://www.legislation.gov.au/F2021L00315/2023-08-04/2023-08-04/text/original/epub/OEBPS/document_1/document_1.html#_Toc143853883> ;
    dcat:landingPage "https://www.legislation.gov.au/F2021L00315/2023-08-04/2023-08-04/text/original/epub/OEBPS/document_1/document_1.html#_Toc143853883"^^xsd:anyURI ;
    dcat:theme legcons:Part .

F2021L00315:88 a legcons:Part,
        owl:Class,
        dcat:Resource ;
    rdfs:label "Part - P88 Part 3 Renewal of registration"@en-AU ;
    dct:hasPart F2021L00315:89,
        F2021L00315:90 ;
    dct:isPartOf F2021L00315:70 ;
    dct:isReferencedBy F2021L00315: ;
    rdfs:comment "Part 3 Renewal of registration - Abrievated Graph Key: P88"@en-AU ;
    skos:broader F2021L00315:89,
        F2021L00315:90 ;
    skos:definition "Part 3 Renewal of registration"@en-AU ;
    skos:narrower F2021L00315:70 ;
    skos:prefLabel "Part P88"@en-AU ;
    dcat:accessURL <https://www.legislation.gov.au/F2021L00315/2023-08-04/2023-08-04/text/original/epub/OEBPS/document_1/document_1.html#_Toc143853912> ;
    dcat:landingPage "https://www.legislation.gov.au/F2021L00315/2023-08-04/2023-08-04/text/original/epub/OEBPS/document_1/document_1.html#_Toc143853912"^^xsd:anyURI ;
    dcat:theme legcons:Part .

F2021L00315:91 a legcons:Part,
        owl:Class,
        dcat:Resource ;
    rdfs:label "Part - P91 Part 4 Variation of registration"@en-AU ;
    dct:hasPart F2021L00315:92,
        F2021L00315:93 ;
    dct:isPartOf F2021L00315:70 ;
    dct:isReferencedBy F2021L00315: ;
    rdfs:comment "Part 4 Variation of registration - Abrievated Graph Key: P91"@en-AU ;
    skos:broader F2021L00315:92,
        F2021L00315:93 ;
    skos:definition "Part 4 Variation of registration"@en-AU ;
    skos:narrower F2021L00315:70 ;
    skos:prefLabel "Part P91"@en-AU ;
    dcat:accessURL <https://www.legislation.gov.au/F2021L00315/2023-08-04/2023-08-04/text/original/epub/OEBPS/document_1/document_1.html#_Toc143853915> ;
    dcat:landingPage "https://www.legislation.gov.au/F2021L00315/2023-08-04/2023-08-04/text/original/epub/OEBPS/document_1/document_1.html#_Toc143853915"^^xsd:anyURI ;
    dcat:theme legcons:Part .

F2021L00315:94 a legcons:Part,
        owl:Class,
        dcat:Resource ;
    rdfs:label "Part - P94 Part 5 Suspension of registration"@en-AU ;
    dct:hasPart F2021L00315:95,
        F2021L00315:97 ;
    dct:isPartOf F2021L00315:70 ;
    dct:isReferencedBy F2021L00315: ;
    rdfs:comment "Part 5 Suspension of registration - Abrievated Graph Key: P94"@en-AU ;
    skos:broader F2021L00315:95,
        F2021L00315:97 ;
    skos:definition "Part 5 Suspension of registration"@en-AU ;
    skos:narrower F2021L00315:70 ;
    skos:prefLabel "Part P94"@en-AU ;
    dcat:accessURL <https://www.legislation.gov.au/F2021L00315/2023-08-04/2023-08-04/text/original/epub/OEBPS/document_1/document_1.html#_Toc143853918> ;
    dcat:landingPage "https://www.legislation.gov.au/F2021L00315/2023-08-04/2023-08-04/text/original/epub/OEBPS/document_1/document_1.html#_Toc143853918"^^xsd:anyURI ;
    dcat:theme legcons:Part .

F2021L00315:99 a legcons:Part,
        owl:Class,
        dcat:Resource ;
    rdfs:label "Part - P99 Part 6 Revocation of registration"@en-AU ;
    dct:hasPart F2021L00315:100,
        F2021L00315:102 ;
    dct:isPartOf F2021L00315:70 ;
    dct:isReferencedBy F2021L00315: ;
    rdfs:comment "Part 6 Revocation of registration - Abrievated Graph Key: P99"@en-AU ;
    skos:broader F2021L00315:100,
        F2021L00315:102 ;
    skos:definition "Part 6 Revocation of registration"@en-AU ;
    skos:narrower F2021L00315:70 ;
    skos:prefLabel "Part P99"@en-AU ;
    dcat:accessURL <https://www.legislation.gov.au/F2021L00315/2023-08-04/2023-08-04/text/original/epub/OEBPS/document_1/document_1.html#_Toc143853923> ;
    dcat:landingPage "https://www.legislation.gov.au/F2021L00315/2023-08-04/2023-08-04/text/original/epub/OEBPS/document_1/document_1.html#_Toc143853923"^^xsd:anyURI ;
    dcat:theme legcons:Part .

F2021L00315:106 a legcons:Part,
        owl:Class,
        dcat:Resource ;
    rdfs:label "Part - P106 Part 8 Matters relating to applications"@en-AU ;
    dct:hasPart F2021L00315:107,
        F2021L00315:108,
        F2021L00315:109 ;
    dct:isPartOf F2021L00315:70 ;
    dct:isReferencedBy F2021L00315: ;
    rdfs:comment "Part 8 Matters relating to applications - Abrievated Graph Key: P106"@en-AU ;
    skos:broader F2021L00315:107,
        F2021L00315:108,
        F2021L00315:109 ;
    skos:definition "Part 8 Matters relating to applications"@en-AU ;
    skos:narrower F2021L00315:70 ;
    skos:prefLabel "Part P106"@en-AU ;
    dcat:accessURL <https://www.legislation.gov.au/F2021L00315/2023-08-04/2023-08-04/text/original/epub/OEBPS/document_1/document_1.html#_Toc143853930> ;
    dcat:landingPage "https://www.legislation.gov.au/F2021L00315/2023-08-04/2023-08-04/text/original/epub/OEBPS/document_1/document_1.html#_Toc143853930"^^xsd:anyURI ;
    dcat:theme legcons:Part .

F2021L00315:110 a legcons:Chapter,
        owl:Class,
        dcat:Resource ;
    rdfs:label "Chapter - C110 Chapter 7 Export permits"@en-AU ;
    dct:hasPart F2021L00315:111,
        F2021L00315:114,
        F2021L00315:119,
        F2021L00315:122 ;
    dct:isReferencedBy F2021L00315: ;
    rdfs:comment "Chapter 7 Export permits - Abrievated Graph Key: C110"@en-AU ;
    skos:broader F2021L00315:111,
        F2021L00315:114,
        F2021L00315:119,
        F2021L00315:122 ;
    skos:definition "Chapter 7 Export permits"@en-AU ;
    skos:prefLabel "Chapter C110"@en-AU ;
    dcat:accessURL <https://www.legislation.gov.au/F2021L00315/2023-08-04/2023-08-04/text/original/epub/OEBPS/document_1/document_1.html#_Toc143853934> ;
    dcat:landingPage "https://www.legislation.gov.au/F2021L00315/2023-08-04/2023-08-04/text/original/epub/OEBPS/document_1/document_1.html#_Toc143853934"^^xsd:anyURI ;
    dcat:theme legcons:Chapter .

F2021L00315:136 a legcons:Part,
        owl:Class,
        dcat:Resource ;
    rdfs:label "Part - P136 Part 3 Official marks"@en-AU ;
    dct:hasPart F2021L00315:137,
        F2021L00315:149,
        F2021L00315:161 ;
    dct:isPartOf F2021L00315:125 ;
    dct:isReferencedBy F2021L00315: ;
    rdfs:comment "Part 3 Official marks - Abrievated Graph Key: P136"@en-AU ;
    skos:broader F2021L00315:137,
        F2021L00315:149,
        F2021L00315:161 ;
    skos:definition "Part 3 Official marks"@en-AU ;
    skos:narrower F2021L00315:125 ;
    skos:prefLabel "Part P136"@en-AU ;
    dcat:accessURL <https://www.legislation.gov.au/F2021L00315/2023-08-04/2023-08-04/text/original/epub/OEBPS/document_1/document_1.html#_Toc143853960> ;
    dcat:landingPage "https://www.legislation.gov.au/F2021L00315/2023-08-04/2023-08-04/text/original/epub/OEBPS/document_1/document_1.html#_Toc143853960"^^xsd:anyURI ;
    dcat:theme legcons:Part .

F2021L00315:248 a legcons:Division,
        owl:Class,
        dcat:Resource ;
    rdfs:label "Division - D248 Division 1 Official marks"@en-AU ;
    dct:hasPart F2021L00315:249,
        F2021L00315:250,
        F2021L00315:251 ;
    dct:isPartOf F2021L00315:247 ;
    dct:isReferencedBy F2021L00315: ;
    rdfs:comment "Division 1 Official marks - Abrievated Graph Key: D248"@en-AU ;
    skos:broader F2021L00315:249,
        F2021L00315:250,
        F2021L00315:251 ;
    skos:definition "Division 1 Official marks"@en-AU ;
    skos:narrower F2021L00315:247 ;
    skos:prefLabel "Division D248"@en-AU ;
    dcat:accessURL <https://www.legislation.gov.au/F2021L00315/2023-08-04/2023-08-04/text/original/epub/OEBPS/document_1/document_1.html#_Toc143854072> ;
    dcat:landingPage "https://www.legislation.gov.au/F2021L00315/2023-08-04/2023-08-04/text/original/epub/OEBPS/document_1/document_1.html#_Toc143854072"^^xsd:anyURI ;
    dcat:theme legcons:Division .

F2021L00315:255 a legcons:Part,
        owl:Class,
        dcat:Resource ;
    rdfs:label "Part - P255 Part 4 Powers and officials"@en-AU ;
    dct:hasPart F2021L00315:256,
        F2021L00315:258,
        F2021L00315:262 ;
    dct:isPartOf F2021L00315:241 ;
    dct:isReferencedBy F2021L00315: ;
    rdfs:comment "Part 4 Powers and officials - Abrievated Graph Key: P255"@en-AU ;
    skos:broader F2021L00315:256,
        F2021L00315:258,
        F2021L00315:262 ;
    skos:definition "Part 4 Powers and officials"@en-AU ;
    skos:narrower F2021L00315:241 ;
    skos:prefLabel "Part P255"@en-AU ;
    dcat:accessURL <https://www.legislation.gov.au/F2021L00315/2023-08-04/2023-08-04/text/original/epub/OEBPS/document_1/document_1.html#_Toc143854079> ;
    dcat:landingPage "https://www.legislation.gov.au/F2021L00315/2023-08-04/2023-08-04/text/original/epub/OEBPS/document_1/document_1.html#_Toc143854079"^^xsd:anyURI ;
    dcat:theme legcons:Part .

F2021L00315:258 a legcons:Division,
        owl:Class,
        dcat:Resource ;
    rdfs:label "Division - D258 Division 2 Bulk vessel approvals"@en-AU ;
    dct:hasPart F2021L00315:259,
        F2021L00315:260,
        F2021L00315:261 ;
    dct:isPartOf F2021L00315:255 ;
    dct:isReferencedBy F2021L00315: ;
    rdfs:comment "Division 2 Bulk vessel approvals - Abrievated Graph Key: D258"@en-AU ;
    skos:broader F2021L00315:259,
        F2021L00315:260,
        F2021L00315:261 ;
    skos:definition "Division 2 Bulk vessel approvals"@en-AU ;
    skos:narrower F2021L00315:255 ;
    skos:prefLabel "Division D258"@en-AU ;
    dcat:accessURL <https://www.legislation.gov.au/F2021L00315/2023-08-04/2023-08-04/text/original/epub/OEBPS/document_1/document_1.html#_Toc143854082> ;
    dcat:landingPage "https://www.legislation.gov.au/F2021L00315/2023-08-04/2023-08-04/text/original/epub/OEBPS/document_1/document_1.html#_Toc143854082"^^xsd:anyURI ;
    dcat:theme legcons:Division .

F2021L00315:66 a legcons:Part,
        owl:Class,
        dcat:Resource ;
    rdfs:label "Part - P66 Part 8 Matters relating to applications"@en-AU ;
    dct:hasPart F2021L00315:67,
        F2021L00315:68,
        F2021L00315:69 ;
    dct:isPartOf F2021L00315:37 ;
    dct:isReferencedBy F2021L00315: ;
    rdfs:comment "Part 8 Matters relating to applications - Abrievated Graph Key: P66"@en-AU ;
    skos:broader F2021L00315:67,
        F2021L00315:68,
        F2021L00315:69 ;
    skos:definition "Part 8 Matters relating to applications"@en-AU ;
    skos:narrower F2021L00315:37 ;
    skos:prefLabel "Part P66"@en-AU ;
    dcat:accessURL <https://www.legislation.gov.au/F2021L00315/2023-08-04/2023-08-04/text/original/epub/OEBPS/document_1/document_1.html#_Toc143853890> ;
    dcat:landingPage "https://www.legislation.gov.au/F2021L00315/2023-08-04/2023-08-04/text/original/epub/OEBPS/document_1/document_1.html#_Toc143853890"^^xsd:anyURI ;
    dcat:theme legcons:Part .

F2021L00315:71 a legcons:Part,
        owl:Class,
        dcat:Resource ;
    rdfs:label "Part - P71 Part 1 Requirements for registration"@en-AU ;
    dct:hasPart F2021L00315:72,
        F2021L00315:73,
        F2021L00315:74 ;
    dct:isPartOf F2021L00315:70 ;
    dct:isReferencedBy F2021L00315: ;
    rdfs:comment "Part 1 Requirements for registration - Abrievated Graph Key: P71"@en-AU ;
    skos:broader F2021L00315:72,
        F2021L00315:73,
        F2021L00315:74 ;
    skos:definition "Part 1 Requirements for registration"@en-AU ;
    skos:narrower F2021L00315:70 ;
    skos:prefLabel "Part P71"@en-AU ;
    dcat:accessURL <https://www.legislation.gov.au/F2021L00315/2023-08-04/2023-08-04/text/original/epub/OEBPS/document_1/document_1.html#_Toc143853895> ;
    dcat:landingPage "https://www.legislation.gov.au/F2021L00315/2023-08-04/2023-08-04/text/original/epub/OEBPS/document_1/document_1.html#_Toc143853895"^^xsd:anyURI ;
    dcat:theme legcons:Part .

F2021L00315:114 a legcons:Part,
        owl:Class,
        dcat:Resource ;
    rdfs:label "Part - P114 Part 2 Variation suspension and revocation of export permit"@en-AU ;
    dct:hasPart F2021L00315:115,
        F2021L00315:116,
        F2021L00315:117,
        F2021L00315:118 ;
    dct:isPartOf F2021L00315:110 ;
    dct:isReferencedBy F2021L00315: ;
    rdfs:comment "Part 2 Variation suspension and revocation of export permit - Abrievated Graph Key: P114"@en-AU ;
    skos:broader F2021L00315:115,
        F2021L00315:116,
        F2021L00315:117,
        F2021L00315:118 ;
    skos:definition "Part 2 Variation suspension and revocation of export permit"@en-AU ;
    skos:narrower F2021L00315:110 ;
    skos:prefLabel "Part P114"@en-AU ;
    dcat:accessURL <https://www.legislation.gov.au/F2021L00315/2023-08-04/2023-08-04/text/original/epub/OEBPS/document_1/document_1.html#_Toc143853938> ;
    dcat:landingPage "https://www.legislation.gov.au/F2021L00315/2023-08-04/2023-08-04/text/original/epub/OEBPS/document_1/document_1.html#_Toc143853938"^^xsd:anyURI ;
    dcat:theme legcons:Part .

F2021L00315:12 a legcons:Part,
        owl:Class,
        dcat:Resource ;
    rdfs:label "Part - P12 Part 1 Goods"@en-AU ;
    dct:hasPart F2021L00315:13,
        F2021L00315:16,
        F2021L00315:17,
        F2021L00315:18 ;
    dct:isPartOf F2021L00315:11 ;
    dct:isReferencedBy F2021L00315: ;
    rdfs:comment "Part 1 Goods - Abrievated Graph Key: P12"@en-AU ;
    skos:broader F2021L00315:13,
        F2021L00315:16,
        F2021L00315:17,
        F2021L00315:18 ;
    skos:definition "Part 1 Goods"@en-AU ;
    skos:narrower F2021L00315:11 ;
    skos:prefLabel "Part P12"@en-AU ;
    dcat:accessURL <https://www.legislation.gov.au/F2021L00315/2023-08-04/2023-08-04/text/original/epub/OEBPS/document_1/document_1.html#_Toc143853836> ;
    dcat:landingPage "https://www.legislation.gov.au/F2021L00315/2023-08-04/2023-08-04/text/original/epub/OEBPS/document_1/document_1.html#_Toc143853836"^^xsd:anyURI ;
    dcat:theme legcons:Part .

F2021L00315:126 a legcons:Part,
        owl:Class,
        dcat:Resource ;
    rdfs:label "Part - P126 Part 1 Notices of intention to export"@en-AU ;
    dct:hasPart F2021L00315:127,
        F2021L00315:128,
        F2021L00315:129,
        F2021L00315:130 ;
    dct:isPartOf F2021L00315:125 ;
    dct:isReferencedBy F2021L00315: ;
    rdfs:comment "Part 1 Notices of intention to export - Abrievated Graph Key: P126"@en-AU ;
    skos:broader F2021L00315:127,
        F2021L00315:128,
        F2021L00315:129,
        F2021L00315:130 ;
    skos:definition "Part 1 Notices of intention to export"@en-AU ;
    skos:narrower F2021L00315:125 ;
    skos:prefLabel "Part P126"@en-AU ;
    dcat:accessURL <https://www.legislation.gov.au/F2021L00315/2023-08-04/2023-08-04/text/original/epub/OEBPS/document_1/document_1.html#_Toc143853950> ;
    dcat:landingPage "https://www.legislation.gov.au/F2021L00315/2023-08-04/2023-08-04/text/original/epub/OEBPS/document_1/document_1.html#_Toc143853950"^^xsd:anyURI ;
    dcat:theme legcons:Part .

F2021L00315:131 a legcons:Part,
        owl:Class,
        dcat:Resource ;
    rdfs:label "Part - P131 Part 2 Trade descriptions"@en-AU ;
    dct:hasPart F2021L00315:132,
        F2021L00315:133,
        F2021L00315:134,
        F2021L00315:135 ;
    dct:isPartOf F2021L00315:125 ;
    dct:isReferencedBy F2021L00315: ;
    rdfs:comment "Part 2 Trade descriptions - Abrievated Graph Key: P131"@en-AU ;
    skos:broader F2021L00315:132,
        F2021L00315:133,
        F2021L00315:134,
        F2021L00315:135 ;
    skos:definition "Part 2 Trade descriptions"@en-AU ;
    skos:narrower F2021L00315:125 ;
    skos:prefLabel "Part P131"@en-AU ;
    dcat:accessURL <https://www.legislation.gov.au/F2021L00315/2023-08-04/2023-08-04/text/original/epub/OEBPS/document_1/document_1.html#_Toc143853955> ;
    dcat:landingPage "https://www.legislation.gov.au/F2021L00315/2023-08-04/2023-08-04/text/original/epub/OEBPS/document_1/document_1.html#_Toc143853955"^^xsd:anyURI ;
    dcat:theme legcons:Part .

F2021L00315:194 a legcons:Part,
        owl:Class,
        dcat:Resource ;
    rdfs:label "Part - P194 Part 4 Authorised officers"@en-AU ;
    dct:hasPart F2021L00315:195,
        F2021L00315:196,
        F2021L00315:197,
        F2021L00315:198 ;
    dct:isPartOf F2021L00315:168 ;
    dct:isReferencedBy F2021L00315: ;
    rdfs:comment "Part 4 Authorised officers - Abrievated Graph Key: P194"@en-AU ;
    skos:broader F2021L00315:195,
        F2021L00315:196,
        F2021L00315:197,
        F2021L00315:198 ;
    skos:definition "Part 4 Authorised officers"@en-AU ;
    skos:narrower F2021L00315:168 ;
    skos:prefLabel "Part P194"@en-AU ;
    dcat:accessURL <https://www.legislation.gov.au/F2021L00315/2023-08-04/2023-08-04/text/original/epub/OEBPS/document_1/document_1.html#_Toc143854018> ;
    dcat:landingPage "https://www.legislation.gov.au/F2021L00315/2023-08-04/2023-08-04/text/original/epub/OEBPS/document_1/document_1.html#_Toc143854018"^^xsd:anyURI ;
    dcat:theme legcons:Part .

F2021L00315:219 a legcons:Chapter,
        owl:Class,
        dcat:Resource ;
    rdfs:label "Chapter - C219 Chapter 11 Miscellaneous"@en-AU ;
    dct:hasPart F2021L00315:220,
        F2021L00315:232,
        F2021L00315:234,
        F2021L00315:237,
        F2021L00315:239 ;
    dct:isReferencedBy F2021L00315: ;
    rdfs:comment "Chapter 11 Miscellaneous - Abrievated Graph Key: C219"@en-AU ;
    skos:broader F2021L00315:220,
        F2021L00315:232,
        F2021L00315:234,
        F2021L00315:237,
        F2021L00315:239 ;
    skos:definition "Chapter 11 Miscellaneous"@en-AU ;
    skos:prefLabel "Chapter C219"@en-AU ;
    dcat:accessURL <https://www.legislation.gov.au/F2021L00315/2023-08-04/2023-08-04/text/original/epub/OEBPS/document_1/document_1.html#_Toc143854043> ;
    dcat:landingPage "https://www.legislation.gov.au/F2021L00315/2023-08-04/2023-08-04/text/original/epub/OEBPS/document_1/document_1.html#_Toc143854043"^^xsd:anyURI ;
    dcat:theme legcons:Chapter .

F2021L00315:241 a legcons:Chapter,
        owl:Class,
        dcat:Resource ;
    rdfs:label "Chapter - C241 Chapter 12 Transitional provisions"@en-AU ;
    dct:hasPart F2021L00315:242,
        F2021L00315:244,
        F2021L00315:247,
        F2021L00315:255,
        F2021L00315:264 ;
    dct:isReferencedBy F2021L00315: ;
    rdfs:comment "Chapter 12 Transitional provisions - Abrievated Graph Key: C241"@en-AU ;
    skos:broader F2021L00315:242,
        F2021L00315:244,
        F2021L00315:247,
        F2021L00315:255,
        F2021L00315:264 ;
    skos:definition "Chapter 12 Transitional provisions"@en-AU ;
    skos:prefLabel "Chapter C241"@en-AU ;
    dcat:accessURL <https://www.legislation.gov.au/F2021L00315/2023-08-04/2023-08-04/text/original/epub/OEBPS/document_1/document_1.html#_Toc143854065> ;
    dcat:landingPage "https://www.legislation.gov.au/F2021L00315/2023-08-04/2023-08-04/text/original/epub/OEBPS/document_1/document_1.html#_Toc143854065"^^xsd:anyURI ;
    dcat:theme legcons:Chapter .

F2021L00315:264 a legcons:Endnotes,
        owl:Class,
        dcat:Resource ;
    rdfs:label "Endnotes - E264 Endnotes"@en-AU ;
    dct:hasPart F2021L00315:265,
        F2021L00315:266,
        F2021L00315:267,
        F2021L00315:268 ;
    dct:isPartOf F2021L00315:241 ;
    dct:isReferencedBy F2021L00315: ;
    rdfs:comment "Endnotes - Abrievated Graph Key: E264"@en-AU ;
    skos:broader F2021L00315:265,
        F2021L00315:266,
        F2021L00315:267,
        F2021L00315:268 ;
    skos:definition "Endnotes"@en-AU ;
    skos:narrower F2021L00315:241 ;
    skos:prefLabel "Endnotes E264"@en-AU ;
    dcat:accessURL <https://www.legislation.gov.au/F2021L00315/2023-08-04/2023-08-04/text/original/epub/OEBPS/document_1/document_1.html#_Toc143854088> ;
    dcat:landingPage "https://www.legislation.gov.au/F2021L00315/2023-08-04/2023-08-04/text/original/epub/OEBPS/document_1/document_1.html#_Toc143854088"^^xsd:anyURI ;
    dcat:theme legcons:Endnotes .

F2021L00315:168 a legcons:Chapter,
        owl:Class,
        dcat:Resource ;
    rdfs:label "Chapter - C168 Chapter 9 Powers and officials"@en-AU ;
    dct:hasPart F2021L00315:169,
        F2021L00315:176,
        F2021L00315:191,
        F2021L00315:194,
        F2021L00315:199,
        F2021L00315:208 ;
    dct:isReferencedBy F2021L00315: ;
    rdfs:comment "Chapter 9 Powers and officials - Abrievated Graph Key: C168"@en-AU ;
    skos:broader F2021L00315:169,
        F2021L00315:176,
        F2021L00315:191,
        F2021L00315:194,
        F2021L00315:199,
        F2021L00315:208 ;
    skos:definition "Chapter 9 Powers and officials"@en-AU ;
    skos:prefLabel "Chapter C168"@en-AU ;
    dcat:accessURL <https://www.legislation.gov.au/F2021L00315/2023-08-04/2023-08-04/text/original/epub/OEBPS/document_1/document_1.html#_Toc143853992> ;
    dcat:landingPage "https://www.legislation.gov.au/F2021L00315/2023-08-04/2023-08-04/text/original/epub/OEBPS/document_1/document_1.html#_Toc143853992"^^xsd:anyURI ;
    dcat:theme legcons:Chapter .

F2021L00315:161 a legcons:Division,
        owl:Class,
        dcat:Resource ;
    rdfs:label "Division - D161 Division 3 Official marking devices"@en-AU ;
    dct:hasPart F2021L00315:162,
        F2021L00315:163,
        F2021L00315:164,
        F2021L00315:165,
        F2021L00315:166,
        F2021L00315:167 ;
    dct:isPartOf F2021L00315:136 ;
    dct:isReferencedBy F2021L00315: ;
    rdfs:comment "Division 3 Official marking devices - Abrievated Graph Key: D161"@en-AU ;
    skos:broader F2021L00315:162,
        F2021L00315:163,
        F2021L00315:164,
        F2021L00315:165,
        F2021L00315:166,
        F2021L00315:167 ;
    skos:definition "Division 3 Official marking devices"@en-AU ;
    skos:narrower F2021L00315:136 ;
    skos:prefLabel "Division D161"@en-AU ;
    dcat:accessURL <https://www.legislation.gov.au/F2021L00315/2023-08-04/2023-08-04/text/original/epub/OEBPS/document_1/document_1.html#_Toc143853985> ;
    dcat:landingPage "https://www.legislation.gov.au/F2021L00315/2023-08-04/2023-08-04/text/original/epub/OEBPS/document_1/document_1.html#_Toc143853985"^^xsd:anyURI ;
    dcat:theme legcons:Division .

F2021L00315:208 a legcons:Part,
        owl:Class,
        dcat:Resource ;
    rdfs:label "Part - P208 Part 6 Container approvals"@en-AU ;
    dct:hasPart F2021L00315:209,
        F2021L00315:210,
        F2021L00315:211,
        F2021L00315:212,
        F2021L00315:213,
        F2021L00315:214,
        F2021L00315:215 ;
    dct:isPartOf F2021L00315:168 ;
    dct:isReferencedBy F2021L00315: ;
    rdfs:comment "Part 6 Container approvals - Abrievated Graph Key: P208"@en-AU ;
    skos:broader F2021L00315:209,
        F2021L00315:210,
        F2021L00315:211,
        F2021L00315:212,
        F2021L00315:213,
        F2021L00315:214,
        F2021L00315:215 ;
    skos:definition "Part 6 Container approvals"@en-AU ;
    skos:narrower F2021L00315:168 ;
    skos:prefLabel "Part P208"@en-AU ;
    dcat:accessURL <https://www.legislation.gov.au/F2021L00315/2023-08-04/2023-08-04/text/original/epub/OEBPS/document_1/document_1.html#_Toc143854032> ;
    dcat:landingPage "https://www.legislation.gov.au/F2021L00315/2023-08-04/2023-08-04/text/original/epub/OEBPS/document_1/document_1.html#_Toc143854032"^^xsd:anyURI ;
    dcat:theme legcons:Part .

F2021L00315:37 a legcons:Chapter,
        owl:Class,
        dcat:Resource ;
    rdfs:label "Chapter - C37 Chapter 3 Accredited properties"@en-AU ;
    dct:hasPart F2021L00315:38,
        F2021L00315:40,
        F2021L00315:48,
        F2021L00315:51,
        F2021L00315:54,
        F2021L00315:59,
        F2021L00315:64,
        F2021L00315:66 ;
    dct:isReferencedBy F2021L00315: ;
    rdfs:comment "Chapter 3 Accredited properties - Abrievated Graph Key: C37"@en-AU ;
    skos:broader F2021L00315:38,
        F2021L00315:40,
        F2021L00315:48,
        F2021L00315:51,
        F2021L00315:54,
        F2021L00315:59,
        F2021L00315:64,
        F2021L00315:66 ;
    skos:definition "Chapter 3 Accredited properties"@en-AU ;
    skos:prefLabel "Chapter C37"@en-AU ;
    dcat:accessURL <https://www.legislation.gov.au/F2021L00315/2023-08-04/2023-08-04/text/original/epub/OEBPS/document_1/document_1.html#_Toc143853861> ;
    dcat:landingPage "https://www.legislation.gov.au/F2021L00315/2023-08-04/2023-08-04/text/original/epub/OEBPS/document_1/document_1.html#_Toc143853861"^^xsd:anyURI ;
    dcat:theme legcons:Chapter .

F2021L00315:40 a legcons:Part,
        owl:Class,
        dcat:Resource ;
    rdfs:label "Part - P40 Part 2 Conditions of accreditation"@en-AU ;
    dct:hasPart F2021L00315:41,
        F2021L00315:42,
        F2021L00315:43,
        F2021L00315:44,
        F2021L00315:45,
        F2021L00315:46,
        F2021L00315:47 ;
    dct:isPartOf F2021L00315:37 ;
    dct:isReferencedBy F2021L00315: ;
    rdfs:comment "Part 2 Conditions of accreditation - Abrievated Graph Key: P40"@en-AU ;
    skos:broader F2021L00315:41,
        F2021L00315:42,
        F2021L00315:43,
        F2021L00315:44,
        F2021L00315:45,
        F2021L00315:46,
        F2021L00315:47 ;
    skos:definition "Part 2 Conditions of accreditation"@en-AU ;
    skos:narrower F2021L00315:37 ;
    skos:prefLabel "Part P40"@en-AU ;
    dcat:accessURL <https://www.legislation.gov.au/F2021L00315/2023-08-04/2023-08-04/text/original/epub/OEBPS/document_1/document_1.html#_Toc143853864> ;
    dcat:landingPage "https://www.legislation.gov.au/F2021L00315/2023-08-04/2023-08-04/text/original/epub/OEBPS/document_1/document_1.html#_Toc143853864"^^xsd:anyURI ;
    dcat:theme legcons:Part .

F2021L00315:70 a legcons:Chapter,
        owl:Class,
        dcat:Resource ;
    rdfs:label "Chapter - C70 Chapter 4 Registered establishments"@en-AU ;
    dct:hasPart F2021L00315:104,
        F2021L00315:106,
        F2021L00315:71,
        F2021L00315:75,
        F2021L00315:88,
        F2021L00315:91,
        F2021L00315:94,
        F2021L00315:99 ;
    dct:isReferencedBy F2021L00315: ;
    rdfs:comment "Chapter 4 Registered establishments - Abrievated Graph Key: C70"@en-AU ;
    skos:broader F2021L00315:104,
        F2021L00315:106,
        F2021L00315:71,
        F2021L00315:75,
        F2021L00315:88,
        F2021L00315:91,
        F2021L00315:94,
        F2021L00315:99 ;
    skos:definition "Chapter 4 Registered establishments"@en-AU ;
    skos:prefLabel "Chapter C70"@en-AU ;
    dcat:accessURL <https://www.legislation.gov.au/F2021L00315/2023-08-04/2023-08-04/text/original/epub/OEBPS/document_1/document_1.html#_Toc143853894> ;
    dcat:landingPage "https://www.legislation.gov.au/F2021L00315/2023-08-04/2023-08-04/text/original/epub/OEBPS/document_1/document_1.html#_Toc143853894"^^xsd:anyURI ;
    dcat:theme legcons:Chapter .

F2021L00315:1 a legcons:Chapter,
        owl:Class,
        dcat:Resource ;
    rdfs:label "Chapter - C1 Chapter 1 Preliminary"@en-AU ;
    dct:hasPart F2021L00315:10,
        F2021L00315:2,
        F2021L00315:3,
        F2021L00315:4,
        F2021L00315:5,
        F2021L00315:6,
        F2021L00315:7,
        F2021L00315:8,
        F2021L00315:9 ;
    dct:isReferencedBy F2021L00315: ;
    rdfs:comment "Chapter 1 Preliminary - Abrievated Graph Key: C1"@en-AU ;
    skos:broader F2021L00315:10,
        F2021L00315:2,
        F2021L00315:3,
        F2021L00315:4,
        F2021L00315:5,
        F2021L00315:6,
        F2021L00315:7,
        F2021L00315:8,
        F2021L00315:9 ;
    skos:definition "Chapter 1 Preliminary"@en-AU ;
    skos:prefLabel "Chapter C1"@en-AU ;
    dcat:accessURL <https://www.legislation.gov.au/F2021L00315/2023-08-04/2023-08-04/text/original/epub/OEBPS/document_1/document_1.html#_Toc143853825> ;
    dcat:landingPage "https://www.legislation.gov.au/F2021L00315/2023-08-04/2023-08-04/text/original/epub/OEBPS/document_1/document_1.html#_Toc143853825"^^xsd:anyURI ;
    dcat:theme legcons:Chapter .

F2021L00315:199 a legcons:Part,
        owl:Class,
        dcat:Resource ;
    rdfs:label "Part - P199 Part 5 Bulk vessel approvals"@en-AU ;
    dct:hasPart F2021L00315:200,
        F2021L00315:201,
        F2021L00315:202,
        F2021L00315:203,
        F2021L00315:204,
        F2021L00315:205,
        F2021L00315:206,
        F2021L00315:207 ;
    dct:isPartOf F2021L00315:168 ;
    dct:isReferencedBy F2021L00315: ;
    rdfs:comment "Part 5 Bulk vessel approvals - Abrievated Graph Key: P199"@en-AU ;
    skos:broader F2021L00315:200,
        F2021L00315:201,
        F2021L00315:202,
        F2021L00315:203,
        F2021L00315:204,
        F2021L00315:205,
        F2021L00315:206,
        F2021L00315:207 ;
    skos:definition "Part 5 Bulk vessel approvals"@en-AU ;
    skos:narrower F2021L00315:168 ;
    skos:prefLabel "Part P199"@en-AU ;
    dcat:accessURL <https://www.legislation.gov.au/F2021L00315/2023-08-04/2023-08-04/text/original/epub/OEBPS/document_1/document_1.html#_Toc143854023> ;
    dcat:landingPage "https://www.legislation.gov.au/F2021L00315/2023-08-04/2023-08-04/text/original/epub/OEBPS/document_1/document_1.html#_Toc143854023"^^xsd:anyURI ;
    dcat:theme legcons:Part .

F2021L00315:180 a legcons:Division,
        owl:Class,
        dcat:Resource ;
    rdfs:label "Division - D180 Division 2 Carrying out assessment etc"@en-AU ;
    dct:hasPart F2021L00315:181,
        F2021L00315:182,
        F2021L00315:183,
        F2021L00315:184,
        F2021L00315:185,
        F2021L00315:186,
        F2021L00315:187,
        F2021L00315:188,
        F2021L00315:189,
        F2021L00315:190 ;
    dct:isPartOf F2021L00315:176 ;
    dct:isReferencedBy F2021L00315: ;
    rdfs:comment "Division 2 Carrying out assessment etc - Abrievated Graph Key: D180"@en-AU ;
    skos:broader F2021L00315:181,
        F2021L00315:182,
        F2021L00315:183,
        F2021L00315:184,
        F2021L00315:185,
        F2021L00315:186,
        F2021L00315:187,
        F2021L00315:188,
        F2021L00315:189,
        F2021L00315:190 ;
    skos:definition "Division 2 Carrying out assessment etc"@en-AU ;
    skos:narrower F2021L00315:176 ;
    skos:prefLabel "Division D180"@en-AU ;
    dcat:accessURL <https://www.legislation.gov.au/F2021L00315/2023-08-04/2023-08-04/text/original/epub/OEBPS/document_1/document_1.html#_Toc143854004> ;
    dcat:landingPage "https://www.legislation.gov.au/F2021L00315/2023-08-04/2023-08-04/text/original/epub/OEBPS/document_1/document_1.html#_Toc143854004"^^xsd:anyURI ;
    dcat:theme legcons:Division .

F2021L00315:11 a legcons:Chapter,
        owl:Class,
        dcat:Resource ;
    rdfs:label "Chapter - C11 Chapter 2 Exporting goods"@en-AU ;
    dct:hasPart F2021L00315:12,
        F2021L00315:19,
        F2021L00315:20,
        F2021L00315:21,
        F2021L00315:22,
        F2021L00315:23,
        F2021L00315:24,
        F2021L00315:25,
        F2021L00315:26,
        F2021L00315:29,
        F2021L00315:32,
        F2021L00315:35 ;
    dct:isReferencedBy F2021L00315: ;
    rdfs:comment "Chapter 2 Exporting goods - Abrievated Graph Key: C11"@en-AU ;
    skos:broader F2021L00315:12,
        F2021L00315:19,
        F2021L00315:20,
        F2021L00315:21,
        F2021L00315:22,
        F2021L00315:23,
        F2021L00315:24,
        F2021L00315:25,
        F2021L00315:26,
        F2021L00315:29,
        F2021L00315:32,
        F2021L00315:35 ;
    skos:definition "Chapter 2 Exporting goods"@en-AU ;
    skos:prefLabel "Chapter C11"@en-AU ;
    dcat:accessURL <https://www.legislation.gov.au/F2021L00315/2023-08-04/2023-08-04/text/original/epub/OEBPS/document_1/document_1.html#_Toc143853835> ;
    dcat:landingPage "https://www.legislation.gov.au/F2021L00315/2023-08-04/2023-08-04/text/original/epub/OEBPS/document_1/document_1.html#_Toc143853835"^^xsd:anyURI ;
    dcat:theme legcons:Chapter .

F2021L00315:137 a legcons:Division,
        owl:Class,
        dcat:Resource ;
    rdfs:label "Division - D137 Division 1 Marks that are official marks"@en-AU ;
    dct:hasPart F2021L00315:138,
        F2021L00315:139,
        F2021L00315:140,
        F2021L00315:141,
        F2021L00315:142,
        F2021L00315:143,
        F2021L00315:144,
        F2021L00315:145,
        F2021L00315:146,
        F2021L00315:147,
        F2021L00315:148 ;
    dct:isPartOf F2021L00315:136 ;
    dct:isReferencedBy F2021L00315: ;
    rdfs:comment "Division 1 Marks that are official marks - Abrievated Graph Key: D137"@en-AU ;
    skos:broader F2021L00315:138,
        F2021L00315:139,
        F2021L00315:140,
        F2021L00315:141,
        F2021L00315:142,
        F2021L00315:143,
        F2021L00315:144,
        F2021L00315:145,
        F2021L00315:146,
        F2021L00315:147,
        F2021L00315:148 ;
    skos:definition "Division 1 Marks that are official marks"@en-AU ;
    skos:narrower F2021L00315:136 ;
    skos:prefLabel "Division D137"@en-AU ;
    dcat:accessURL <https://www.legislation.gov.au/F2021L00315/2023-08-04/2023-08-04/text/original/epub/OEBPS/document_1/document_1.html#_Toc143853961> ;
    dcat:landingPage "https://www.legislation.gov.au/F2021L00315/2023-08-04/2023-08-04/text/original/epub/OEBPS/document_1/document_1.html#_Toc143853961"^^xsd:anyURI ;
    dcat:theme legcons:Division .

F2021L00315:149 a legcons:Division,
        owl:Class,
        dcat:Resource ;
    rdfs:label "Division - D149 Division 2 General rules relating to official marks"@en-AU ;
    dct:hasPart F2021L00315:150,
        F2021L00315:151,
        F2021L00315:152,
        F2021L00315:153,
        F2021L00315:154,
        F2021L00315:155,
        F2021L00315:156,
        F2021L00315:157,
        F2021L00315:158,
        F2021L00315:159,
        F2021L00315:160 ;
    dct:isPartOf F2021L00315:136 ;
    dct:isReferencedBy F2021L00315: ;
    rdfs:comment "Division 2 General rules relating to official marks - Abrievated Graph Key: D149"@en-AU ;
    skos:broader F2021L00315:150,
        F2021L00315:151,
        F2021L00315:152,
        F2021L00315:153,
        F2021L00315:154,
        F2021L00315:155,
        F2021L00315:156,
        F2021L00315:157,
        F2021L00315:158,
        F2021L00315:159,
        F2021L00315:160 ;
    skos:definition "Division 2 General rules relating to official marks"@en-AU ;
    skos:narrower F2021L00315:136 ;
    skos:prefLabel "Division D149"@en-AU ;
    dcat:accessURL <https://www.legislation.gov.au/F2021L00315/2023-08-04/2023-08-04/text/original/epub/OEBPS/document_1/document_1.html#_Toc143853973> ;
    dcat:landingPage "https://www.legislation.gov.au/F2021L00315/2023-08-04/2023-08-04/text/original/epub/OEBPS/document_1/document_1.html#_Toc143853973"^^xsd:anyURI ;
    dcat:theme legcons:Division .

F2021L00315:220 a legcons:Part,
        owl:Class,
        dcat:Resource ;
    rdfs:label "Part - P220 Part 1 Records"@en-AU ;
    dct:hasPart F2021L00315:221,
        F2021L00315:222,
        F2021L00315:223,
        F2021L00315:224,
        F2021L00315:225,
        F2021L00315:226,
        F2021L00315:227,
        F2021L00315:228,
        F2021L00315:229,
        F2021L00315:230,
        F2021L00315:231 ;
    dct:isPartOf F2021L00315:219 ;
    dct:isReferencedBy F2021L00315: ;
    rdfs:comment "Part 1 Records - Abrievated Graph Key: P220"@en-AU ;
    skos:broader F2021L00315:221,
        F2021L00315:222,
        F2021L00315:223,
        F2021L00315:224,
        F2021L00315:225,
        F2021L00315:226,
        F2021L00315:227,
        F2021L00315:228,
        F2021L00315:229,
        F2021L00315:230,
        F2021L00315:231 ;
    skos:definition "Part 1 Records"@en-AU ;
    skos:narrower F2021L00315:219 ;
    skos:prefLabel "Part P220"@en-AU ;
    dcat:accessURL <https://www.legislation.gov.au/F2021L00315/2023-08-04/2023-08-04/text/original/epub/OEBPS/document_1/document_1.html#_Toc143854044> ;
    dcat:landingPage "https://www.legislation.gov.au/F2021L00315/2023-08-04/2023-08-04/text/original/epub/OEBPS/document_1/document_1.html#_Toc143854044"^^xsd:anyURI ;
    dcat:theme legcons:Part .

F2021L00315:75 a legcons:Part,
        owl:Class,
        dcat:Resource ;
    rdfs:label "Part - P75 Part 2 Conditions of registration"@en-AU ;
    dct:hasPart F2021L00315:76,
        F2021L00315:77,
        F2021L00315:78,
        F2021L00315:79,
        F2021L00315:80,
        F2021L00315:81,
        F2021L00315:82,
        F2021L00315:83,
        F2021L00315:84,
        F2021L00315:85,
        F2021L00315:86,
        F2021L00315:87 ;
    dct:isPartOf F2021L00315:70 ;
    dct:isReferencedBy F2021L00315: ;
    rdfs:comment "Part 2 Conditions of registration - Abrievated Graph Key: P75"@en-AU ;
    skos:broader F2021L00315:76,
        F2021L00315:77,
        F2021L00315:78,
        F2021L00315:79,
        F2021L00315:80,
        F2021L00315:81,
        F2021L00315:82,
        F2021L00315:83,
        F2021L00315:84,
        F2021L00315:85,
        F2021L00315:86,
        F2021L00315:87 ;
    skos:definition "Part 2 Conditions of registration"@en-AU ;
    skos:narrower F2021L00315:70 ;
    skos:prefLabel "Part P75"@en-AU ;
    dcat:accessURL <https://www.legislation.gov.au/F2021L00315/2023-08-04/2023-08-04/text/original/epub/OEBPS/document_1/document_1.html#_Toc143853899> ;
    dcat:landingPage "https://www.legislation.gov.au/F2021L00315/2023-08-04/2023-08-04/text/original/epub/OEBPS/document_1/document_1.html#_Toc143853899"^^xsd:anyURI ;
    dcat:theme legcons:Part .

F2021L00315: a owl:Class,
        dcat:Dataset,
        dcat:Resource ;
    rdfs:label "Export Control (Plants and Plant Products) Rules 2021" ;
    dct:Jurisdiction " Department of Agriculture, Fisheries and Forestry "@en-AU ;
    dct:created "2024-08-30T15:13:24.761579"^^xsd:dateTime ;
    dct:creator "https://orcid.org/0009-0007-8434-7325"^^xsd:anyURI ;
    dct:date "2023-08-04T00:00:00+10:00"^^xsd:dateTime ;
    dct:description "Export Control (Plants and Plant Products) Rules 2021"@en-AU ;
    dct:identifier "https://www.legislation.gov.au/F2021L00315/latest"^^xsd:anyURI ;
    dct:license <https://creativecommons.org/licenses/by-sa/4.0/> ;
    dct:source "scheme=AGLSTERMS.AglsAgent; corporateName=Office Parliamentary Counsel; address=Locked Bag 30 Kingston ACT 2604; contact=+61 2 6120 1400"@en-AU ;
    dct:subject "Export Control (Plants and Plant Products) Rules 2021"@en-AU ;
    dct:title "Export Control (Plants and Plant Products) Rules 2021"@en-AU ;
    owl:imports legcons: ;
    dcat:theme legcons:Chapter,
        legcons:Division,
        legcons:Endnotes,
        legcons:Item,
        legcons:Part ;
    schema:identifier "F2021L00315" ;
    schema:status "In force" ;
    schema:version "F2023C00759 (C03)" .

