@prefix F2021L00313: <http://example.org/au/leg/dataset/F2021L00313/> .
@prefix dcat: <http://www.w3.org/ns/dcat#> .
@prefix dct: <http://purl.org/dc/terms/> .
@prefix legcons: <http://example.org/au/leg/concepts/> .
@prefix owl: <http://www.w3.org/2002/07/owl#> .
@prefix rdfs: <http://www.w3.org/2000/01/rdf-schema#> .
@prefix schema: <https://schema.org/> .
@prefix skos: <http://www.w3.org/2004/02/skos/core#> .
@prefix xsd: <http://www.w3.org/2001/XMLSchema#> .

F2021L00313:10 a legcons:Division,
        owl:Class,
        dcat:Resource ;
    rdfs:label "Division - D10 Division 2 Other interpretation provisions"@en-AU ;
    dct:isPartOf F2021L00313:1 ;
    dct:isReferencedBy F2021L00313: ;
    rdfs:comment "Division 2 Other interpretation provisions - Abrievated Graph Key: D10"@en-AU ;
    skos:definition "Division 2 Other interpretation provisions"@en-AU ;
    skos:narrower F2021L00313:1 ;
    skos:prefLabel "Division D10"@en-AU ;
    dcat:accessURL <https://www.legislation.gov.au/F2021L00313/2023-08-04/2023-08-04/text/original/epub/OEBPS/document_1/document_1.html#_Toc144217855> ;
    dcat:landingPage "https://www.legislation.gov.au/F2021L00313/2023-08-04/2023-08-04/text/original/epub/OEBPS/document_1/document_1.html#_Toc144217855"^^xsd:anyURI ;
    dcat:theme legcons:Division .

F2021L00313:100 a legcons:Item,
        owl:Class,
        dcat:Resource ;
    rdfs:label "Item - I100 5 16  Trade description must be applied to prescribed wild game meat and wild game meat products that are intended to be exported"@en-AU ;
    dct:isPartOf F2021L00313:99 ;
    dct:isReferencedBy F2021L00313: ;
    rdfs:comment "5 16  Trade description must be applied to prescribed wild game meat and wild game meat products that are intended to be exported - Abrievated Graph Key: I100"@en-AU ;
    skos:definition "5 16  Trade description must be applied to prescribed wild game meat and wild game meat products that are intended to be exported"@en-AU ;
    skos:narrower F2021L00313:99 ;
    skos:prefLabel "Item I100"@en-AU ;
    dcat:accessURL <https://www.legislation.gov.au/F2021L00313/2023-08-04/2023-08-04/text/original/epub/OEBPS/document_1/document_1.html#_Toc144217945> ;
    dcat:landingPage "https://www.legislation.gov.au/F2021L00313/2023-08-04/2023-08-04/text/original/epub/OEBPS/document_1/document_1.html#_Toc144217945"^^xsd:anyURI ;
    dcat:theme legcons:Item .

F2021L00313:101 a legcons:Item,
        owl:Class,
        dcat:Resource ;
    rdfs:label "Item - I101 5 17  Prescribed wild game meat or wild game meat products in cartons or cans"@en-AU ;
    dct:isPartOf F2021L00313:99 ;
    dct:isReferencedBy F2021L00313: ;
    rdfs:comment "5 17  Prescribed wild game meat or wild game meat products in cartons or cans - Abrievated Graph Key: I101"@en-AU ;
    skos:definition "5 17  Prescribed wild game meat or wild game meat products in cartons or cans"@en-AU ;
    skos:narrower F2021L00313:99 ;
    skos:prefLabel "Item I101"@en-AU ;
    dcat:accessURL <https://www.legislation.gov.au/F2021L00313/2023-08-04/2023-08-04/text/original/epub/OEBPS/document_1/document_1.html#_Toc144217946> ;
    dcat:landingPage "https://www.legislation.gov.au/F2021L00313/2023-08-04/2023-08-04/text/original/epub/OEBPS/document_1/document_1.html#_Toc144217946"^^xsd:anyURI ;
    dcat:theme legcons:Item .

F2021L00313:103 a legcons:Item,
        owl:Class,
        dcat:Resource ;
    rdfs:label "Item - I103 5 18  References to particular official marks"@en-AU ;
    dct:isPartOf F2021L00313:102 ;
    dct:isReferencedBy F2021L00313: ;
    rdfs:comment "5 18  References to particular official marks - Abrievated Graph Key: I103"@en-AU ;
    skos:definition "5 18  References to particular official marks"@en-AU ;
    skos:narrower F2021L00313:102 ;
    skos:prefLabel "Item I103"@en-AU ;
    dcat:accessURL <https://www.legislation.gov.au/F2021L00313/2023-08-04/2023-08-04/text/original/epub/OEBPS/document_1/document_1.html#_Toc144217948> ;
    dcat:landingPage "https://www.legislation.gov.au/F2021L00313/2023-08-04/2023-08-04/text/original/epub/OEBPS/document_1/document_1.html#_Toc144217948"^^xsd:anyURI ;
    dcat:theme legcons:Item .

F2021L00313:104 a legcons:Item,
        owl:Class,
        dcat:Resource ;
    rdfs:label "Item - I104 5 19  Carcases and carcase parts"@en-AU ;
    dct:isPartOf F2021L00313:102 ;
    dct:isReferencedBy F2021L00313: ;
    rdfs:comment "5 19  Carcases and carcase parts - Abrievated Graph Key: I104"@en-AU ;
    skos:definition "5 19  Carcases and carcase parts"@en-AU ;
    skos:narrower F2021L00313:102 ;
    skos:prefLabel "Item I104"@en-AU ;
    dcat:accessURL <https://www.legislation.gov.au/F2021L00313/2023-08-04/2023-08-04/text/original/epub/OEBPS/document_1/document_1.html#_Toc144217949> ;
    dcat:landingPage "https://www.legislation.gov.au/F2021L00313/2023-08-04/2023-08-04/text/original/epub/OEBPS/document_1/document_1.html#_Toc144217949"^^xsd:anyURI ;
    dcat:theme legcons:Item .

F2021L00313:105 a legcons:Item,
        owl:Class,
        dcat:Resource ;
    rdfs:label "Item - I105 5 20  Cartons containing prescribed wild game meat or wild game meat products"@en-AU ;
    dct:isPartOf F2021L00313:102 ;
    dct:isReferencedBy F2021L00313: ;
    rdfs:comment "5 20  Cartons containing prescribed wild game meat or wild game meat products - Abrievated Graph Key: I105"@en-AU ;
    skos:definition "5 20  Cartons containing prescribed wild game meat or wild game meat products"@en-AU ;
    skos:narrower F2021L00313:102 ;
    skos:prefLabel "Item I105"@en-AU ;
    dcat:accessURL <https://www.legislation.gov.au/F2021L00313/2023-08-04/2023-08-04/text/original/epub/OEBPS/document_1/document_1.html#_Toc144217950> ;
    dcat:landingPage "https://www.legislation.gov.au/F2021L00313/2023-08-04/2023-08-04/text/original/epub/OEBPS/document_1/document_1.html#_Toc144217950"^^xsd:anyURI ;
    dcat:theme legcons:Item .

F2021L00313:106 a legcons:Item,
        owl:Class,
        dcat:Resource ;
    rdfs:label "Item - I106 5 21  State or Territory classification marks must not be applied"@en-AU ;
    dct:isPartOf F2021L00313:102 ;
    dct:isReferencedBy F2021L00313: ;
    rdfs:comment "5 21  State or Territory classification marks must not be applied - Abrievated Graph Key: I106"@en-AU ;
    skos:definition "5 21  State or Territory classification marks must not be applied"@en-AU ;
    skos:narrower F2021L00313:102 ;
    skos:prefLabel "Item I106"@en-AU ;
    dcat:accessURL <https://www.legislation.gov.au/F2021L00313/2023-08-04/2023-08-04/text/original/epub/OEBPS/document_1/document_1.html#_Toc144217951> ;
    dcat:landingPage "https://www.legislation.gov.au/F2021L00313/2023-08-04/2023-08-04/text/original/epub/OEBPS/document_1/document_1.html#_Toc144217951"^^xsd:anyURI ;
    dcat:theme legcons:Item .

F2021L00313:108 a legcons:Item,
        owl:Class,
        dcat:Resource ;
    rdfs:label "Item - I108 5 22  Segregation identification security and traceabilitygeneral"@en-AU ;
    dct:isPartOf F2021L00313:107 ;
    dct:isReferencedBy F2021L00313: ;
    rdfs:comment "5 22  Segregation identification security and traceabilitygeneral - Abrievated Graph Key: I108"@en-AU ;
    skos:definition "5 22  Segregation identification security and traceabilitygeneral"@en-AU ;
    skos:narrower F2021L00313:107 ;
    skos:prefLabel "Item I108"@en-AU ;
    dcat:accessURL <https://www.legislation.gov.au/F2021L00313/2023-08-04/2023-08-04/text/original/epub/OEBPS/document_1/document_1.html#_Toc144217953> ;
    dcat:landingPage "https://www.legislation.gov.au/F2021L00313/2023-08-04/2023-08-04/text/original/epub/OEBPS/document_1/document_1.html#_Toc144217953"^^xsd:anyURI ;
    dcat:theme legcons:Item .

F2021L00313:109 a legcons:Item,
        owl:Class,
        dcat:Resource ;
    rdfs:label "Item - I109 5 23  Establishments where wild game meat or wild game meat products that are not for export etc are prepared"@en-AU ;
    dct:isPartOf F2021L00313:107 ;
    dct:isReferencedBy F2021L00313: ;
    rdfs:comment "5 23  Establishments where wild game meat or wild game meat products that are not for export etc are prepared - Abrievated Graph Key: I109"@en-AU ;
    skos:definition "5 23  Establishments where wild game meat or wild game meat products that are not for export etc are prepared"@en-AU ;
    skos:narrower F2021L00313:107 ;
    skos:prefLabel "Item I109"@en-AU ;
    dcat:accessURL <https://www.legislation.gov.au/F2021L00313/2023-08-04/2023-08-04/text/original/epub/OEBPS/document_1/document_1.html#_Toc144217954> ;
    dcat:landingPage "https://www.legislation.gov.au/F2021L00313/2023-08-04/2023-08-04/text/original/epub/OEBPS/document_1/document_1.html#_Toc144217954"^^xsd:anyURI ;
    dcat:theme legcons:Item .

F2021L00313:11 a legcons:Item,
        owl:Class,
        dcat:Resource ;
    rdfs:label "Item - I11 1 7  References to authorised officer and meat safety inspector"@en-AU ;
    dct:isPartOf F2021L00313:1 ;
    dct:isReferencedBy F2021L00313: ;
    rdfs:comment "1 7  References to authorised officer and meat safety inspector - Abrievated Graph Key: I11"@en-AU ;
    skos:definition "1 7  References to authorised officer and meat safety inspector"@en-AU ;
    skos:narrower F2021L00313:1 ;
    skos:prefLabel "Item I11"@en-AU ;
    dcat:accessURL <https://www.legislation.gov.au/F2021L00313/2023-08-04/2023-08-04/text/original/epub/OEBPS/document_1/document_1.html#_Toc144217856> ;
    dcat:landingPage "https://www.legislation.gov.au/F2021L00313/2023-08-04/2023-08-04/text/original/epub/OEBPS/document_1/document_1.html#_Toc144217856"^^xsd:anyURI ;
    dcat:theme legcons:Item .

F2021L00313:110 a legcons:Item,
        owl:Class,
        dcat:Resource ;
    rdfs:label "Item - I110 5 24  Integritygeneral"@en-AU ;
    dct:isPartOf F2021L00313:107 ;
    dct:isReferencedBy F2021L00313: ;
    rdfs:comment "5 24  Integritygeneral - Abrievated Graph Key: I110"@en-AU ;
    skos:definition "5 24  Integritygeneral"@en-AU ;
    skos:narrower F2021L00313:107 ;
    skos:prefLabel "Item I110"@en-AU ;
    dcat:accessURL <https://www.legislation.gov.au/F2021L00313/2023-08-04/2023-08-04/text/original/epub/OEBPS/document_1/document_1.html#_Toc144217955> ;
    dcat:landingPage "https://www.legislation.gov.au/F2021L00313/2023-08-04/2023-08-04/text/original/epub/OEBPS/document_1/document_1.html#_Toc144217955"^^xsd:anyURI ;
    dcat:theme legcons:Item .

F2021L00313:111 a legcons:Item,
        owl:Class,
        dcat:Resource ;
    rdfs:label "Item - I111 5 25  Identificationtype of animal"@en-AU ;
    dct:isPartOf F2021L00313:107 ;
    dct:isReferencedBy F2021L00313: ;
    rdfs:comment "5 25  Identificationtype of animal - Abrievated Graph Key: I111"@en-AU ;
    skos:definition "5 25  Identificationtype of animal"@en-AU ;
    skos:narrower F2021L00313:107 ;
    skos:prefLabel "Item I111"@en-AU ;
    dcat:accessURL <https://www.legislation.gov.au/F2021L00313/2023-08-04/2023-08-04/text/original/epub/OEBPS/document_1/document_1.html#_Toc144217956> ;
    dcat:landingPage "https://www.legislation.gov.au/F2021L00313/2023-08-04/2023-08-04/text/original/epub/OEBPS/document_1/document_1.html#_Toc144217956"^^xsd:anyURI ;
    dcat:theme legcons:Item .

F2021L00313:112 a legcons:Item,
        owl:Class,
        dcat:Resource ;
    rdfs:label "Item - I112 5 26  Export market eligibility"@en-AU ;
    dct:isPartOf F2021L00313:107 ;
    dct:isReferencedBy F2021L00313: ;
    rdfs:comment "5 26  Export market eligibility - Abrievated Graph Key: I112"@en-AU ;
    skos:definition "5 26  Export market eligibility"@en-AU ;
    skos:narrower F2021L00313:107 ;
    skos:prefLabel "Item I112"@en-AU ;
    dcat:accessURL <https://www.legislation.gov.au/F2021L00313/2023-08-04/2023-08-04/text/original/epub/OEBPS/document_1/document_1.html#_Toc144217957> ;
    dcat:landingPage "https://www.legislation.gov.au/F2021L00313/2023-08-04/2023-08-04/text/original/epub/OEBPS/document_1/document_1.html#_Toc144217957"^^xsd:anyURI ;
    dcat:theme legcons:Item .

F2021L00313:113 a legcons:Item,
        owl:Class,
        dcat:Resource ;
    rdfs:label "Item - I113 5 27  Action if prescribed wild game meat or wild game meat products are unwholesome or integrity etc cannot be ensured"@en-AU ;
    dct:isPartOf F2021L00313:107 ;
    dct:isReferencedBy F2021L00313: ;
    rdfs:comment "5 27  Action if prescribed wild game meat or wild game meat products are unwholesome or integrity etc cannot be ensured - Abrievated Graph Key: I113"@en-AU ;
    skos:definition "5 27  Action if prescribed wild game meat or wild game meat products are unwholesome or integrity etc cannot be ensured"@en-AU ;
    skos:narrower F2021L00313:107 ;
    skos:prefLabel "Item I113"@en-AU ;
    dcat:accessURL <https://www.legislation.gov.au/F2021L00313/2023-08-04/2023-08-04/text/original/epub/OEBPS/document_1/document_1.html#_Toc144217958> ;
    dcat:landingPage "https://www.legislation.gov.au/F2021L00313/2023-08-04/2023-08-04/text/original/epub/OEBPS/document_1/document_1.html#_Toc144217958"^^xsd:anyURI ;
    dcat:theme legcons:Item .

F2021L00313:115 a legcons:Item,
        owl:Class,
        dcat:Resource ;
    rdfs:label "Item - I115 5 28  Information and declarations relating to transferred prescribed wild game meat or wild game meat products"@en-AU ;
    dct:isPartOf F2021L00313:114 ;
    dct:isReferencedBy F2021L00313: ;
    rdfs:comment "5 28  Information and declarations relating to transferred prescribed wild game meat or wild game meat products - Abrievated Graph Key: I115"@en-AU ;
    skos:definition "5 28  Information and declarations relating to transferred prescribed wild game meat or wild game meat products"@en-AU ;
    skos:narrower F2021L00313:114 ;
    skos:prefLabel "Item I115"@en-AU ;
    dcat:accessURL <https://www.legislation.gov.au/F2021L00313/2023-08-04/2023-08-04/text/original/epub/OEBPS/document_1/document_1.html#_Toc144217960> ;
    dcat:landingPage "https://www.legislation.gov.au/F2021L00313/2023-08-04/2023-08-04/text/original/epub/OEBPS/document_1/document_1.html#_Toc144217960"^^xsd:anyURI ;
    dcat:theme legcons:Item .

F2021L00313:116 a legcons:Item,
        owl:Class,
        dcat:Resource ;
    rdfs:label "Item - I116 5 29  Information and declarations not received or inaccurate or incomplete"@en-AU ;
    dct:isPartOf F2021L00313:114 ;
    dct:isReferencedBy F2021L00313: ;
    rdfs:comment "5 29  Information and declarations not received or inaccurate or incomplete - Abrievated Graph Key: I116"@en-AU ;
    skos:definition "5 29  Information and declarations not received or inaccurate or incomplete"@en-AU ;
    skos:narrower F2021L00313:114 ;
    skos:prefLabel "Item I116"@en-AU ;
    dcat:accessURL <https://www.legislation.gov.au/F2021L00313/2023-08-04/2023-08-04/text/original/epub/OEBPS/document_1/document_1.html#_Toc144217961> ;
    dcat:landingPage "https://www.legislation.gov.au/F2021L00313/2023-08-04/2023-08-04/text/original/epub/OEBPS/document_1/document_1.html#_Toc144217961"^^xsd:anyURI ;
    dcat:theme legcons:Item .

F2021L00313:118 a legcons:Item,
        owl:Class,
        dcat:Resource ;
    rdfs:label "Item - I118 5 30  Authorised officer must be present while certain export operations are carried out"@en-AU ;
    dct:isPartOf F2021L00313:117 ;
    dct:isReferencedBy F2021L00313: ;
    rdfs:comment "5 30  Authorised officer must be present while certain export operations are carried out - Abrievated Graph Key: I118"@en-AU ;
    skos:definition "5 30  Authorised officer must be present while certain export operations are carried out"@en-AU ;
    skos:narrower F2021L00313:117 ;
    skos:prefLabel "Item I118"@en-AU ;
    dcat:accessURL <https://www.legislation.gov.au/F2021L00313/2023-08-04/2023-08-04/text/original/epub/OEBPS/document_1/document_1.html#_Toc144217963> ;
    dcat:landingPage "https://www.legislation.gov.au/F2021L00313/2023-08-04/2023-08-04/text/original/epub/OEBPS/document_1/document_1.html#_Toc144217963"^^xsd:anyURI ;
    dcat:theme legcons:Item .

F2021L00313:12 a legcons:Item,
        owl:Class,
        dcat:Resource ;
    rdfs:label "Item - I12 1 8  Modifications of certain terms used in the Australian Meat Standard"@en-AU ;
    dct:isPartOf F2021L00313:1 ;
    dct:isReferencedBy F2021L00313: ;
    rdfs:comment "1 8  Modifications of certain terms used in the Australian Meat Standard - Abrievated Graph Key: I12"@en-AU ;
    skos:definition "1 8  Modifications of certain terms used in the Australian Meat Standard"@en-AU ;
    skos:narrower F2021L00313:1 ;
    skos:prefLabel "Item I12"@en-AU ;
    dcat:accessURL <https://www.legislation.gov.au/F2021L00313/2023-08-04/2023-08-04/text/original/epub/OEBPS/document_1/document_1.html#_Toc144217857> ;
    dcat:landingPage "https://www.legislation.gov.au/F2021L00313/2023-08-04/2023-08-04/text/original/epub/OEBPS/document_1/document_1.html#_Toc144217857"^^xsd:anyURI ;
    dcat:theme legcons:Item .

F2021L00313:120 a legcons:Item,
        owl:Class,
        dcat:Resource ;
    rdfs:label "Item - I120 5 31  Management practices organisational structure resources and personnel"@en-AU ;
    dct:isPartOf F2021L00313:119 ;
    dct:isReferencedBy F2021L00313: ;
    rdfs:comment "5 31  Management practices organisational structure resources and personnel - Abrievated Graph Key: I120"@en-AU ;
    skos:definition "5 31  Management practices organisational structure resources and personnel"@en-AU ;
    skos:narrower F2021L00313:119 ;
    skos:prefLabel "Item I120"@en-AU ;
    dcat:accessURL <https://www.legislation.gov.au/F2021L00313/2023-08-04/2023-08-04/text/original/epub/OEBPS/document_1/document_1.html#_Toc144217965> ;
    dcat:landingPage "https://www.legislation.gov.au/F2021L00313/2023-08-04/2023-08-04/text/original/epub/OEBPS/document_1/document_1.html#_Toc144217965"^^xsd:anyURI ;
    dcat:theme legcons:Item .

F2021L00313:121 a legcons:Item,
        owl:Class,
        dcat:Resource ;
    rdfs:label "Item - I121 5 32  Verification of compliance with the Act and other matters"@en-AU ;
    dct:isPartOf F2021L00313:119 ;
    dct:isReferencedBy F2021L00313: ;
    rdfs:comment "5 32  Verification of compliance with the Act and other matters - Abrievated Graph Key: I121"@en-AU ;
    skos:definition "5 32  Verification of compliance with the Act and other matters"@en-AU ;
    skos:narrower F2021L00313:119 ;
    skos:prefLabel "Item I121"@en-AU ;
    dcat:accessURL <https://www.legislation.gov.au/F2021L00313/2023-08-04/2023-08-04/text/original/epub/OEBPS/document_1/document_1.html#_Toc144217966> ;
    dcat:landingPage "https://www.legislation.gov.au/F2021L00313/2023-08-04/2023-08-04/text/original/epub/OEBPS/document_1/document_1.html#_Toc144217966"^^xsd:anyURI ;
    dcat:theme legcons:Item .

F2021L00313:122 a legcons:Item,
        owl:Class,
        dcat:Resource ;
    rdfs:label "Item - I122 5 33  Action must be taken to address non compliance"@en-AU ;
    dct:isPartOf F2021L00313:119 ;
    dct:isReferencedBy F2021L00313: ;
    rdfs:comment "5 33  Action must be taken to address non compliance - Abrievated Graph Key: I122"@en-AU ;
    skos:definition "5 33  Action must be taken to address non compliance"@en-AU ;
    skos:narrower F2021L00313:119 ;
    skos:prefLabel "Item I122"@en-AU ;
    dcat:accessURL <https://www.legislation.gov.au/F2021L00313/2023-08-04/2023-08-04/text/original/epub/OEBPS/document_1/document_1.html#_Toc144217967> ;
    dcat:landingPage "https://www.legislation.gov.au/F2021L00313/2023-08-04/2023-08-04/text/original/epub/OEBPS/document_1/document_1.html#_Toc144217967"^^xsd:anyURI ;
    dcat:theme legcons:Item .

F2021L00313:123 a legcons:Item,
        owl:Class,
        dcat:Resource ;
    rdfs:label "Item - I123 5 34  Internal audit and management review"@en-AU ;
    dct:isPartOf F2021L00313:119 ;
    dct:isReferencedBy F2021L00313: ;
    rdfs:comment "5 34  Internal audit and management review - Abrievated Graph Key: I123"@en-AU ;
    skos:definition "5 34  Internal audit and management review"@en-AU ;
    skos:narrower F2021L00313:119 ;
    skos:prefLabel "Item I123"@en-AU ;
    dcat:accessURL <https://www.legislation.gov.au/F2021L00313/2023-08-04/2023-08-04/text/original/epub/OEBPS/document_1/document_1.html#_Toc144217968> ;
    dcat:landingPage "https://www.legislation.gov.au/F2021L00313/2023-08-04/2023-08-04/text/original/epub/OEBPS/document_1/document_1.html#_Toc144217968"^^xsd:anyURI ;
    dcat:theme legcons:Item .

F2021L00313:125 a legcons:Item,
        owl:Class,
        dcat:Resource ;
    rdfs:label "Item - I125 5 35  Period within which application to renew approved arrangement must be made"@en-AU ;
    dct:isPartOf F2021L00313:124 ;
    dct:isReferencedBy F2021L00313: ;
    rdfs:comment "5 35  Period within which application to renew approved arrangement must be made - Abrievated Graph Key: I125"@en-AU ;
    skos:definition "5 35  Period within which application to renew approved arrangement must be made"@en-AU ;
    skos:narrower F2021L00313:124 ;
    skos:prefLabel "Item I125"@en-AU ;
    dcat:accessURL <https://www.legislation.gov.au/F2021L00313/2023-08-04/2023-08-04/text/original/epub/OEBPS/document_1/document_1.html#_Toc144217970> ;
    dcat:landingPage "https://www.legislation.gov.au/F2021L00313/2023-08-04/2023-08-04/text/original/epub/OEBPS/document_1/document_1.html#_Toc144217970"^^xsd:anyURI ;
    dcat:theme legcons:Item .

F2021L00313:128 a legcons:Item,
        owl:Class,
        dcat:Resource ;
    rdfs:label "Item - I128 5 36  Requirements that must be met for variation to be approved or conditions varied"@en-AU ;
    dct:isPartOf F2021L00313:127 ;
    dct:isReferencedBy F2021L00313: ;
    rdfs:comment "5 36  Requirements that must be met for variation to be approved or conditions varied - Abrievated Graph Key: I128"@en-AU ;
    skos:definition "5 36  Requirements that must be met for variation to be approved or conditions varied"@en-AU ;
    skos:narrower F2021L00313:127 ;
    skos:prefLabel "Item I128"@en-AU ;
    dcat:accessURL <https://www.legislation.gov.au/F2021L00313/2023-08-04/2023-08-04/text/original/epub/OEBPS/document_1/document_1.html#_Toc144217973> ;
    dcat:landingPage "https://www.legislation.gov.au/F2021L00313/2023-08-04/2023-08-04/text/original/epub/OEBPS/document_1/document_1.html#_Toc144217973"^^xsd:anyURI ;
    dcat:theme legcons:Item .

F2021L00313:129 a legcons:Item,
        owl:Class,
        dcat:Resource ;
    rdfs:label "Item - I129 5 37  Significant variations"@en-AU ;
    dct:isPartOf F2021L00313:127 ;
    dct:isReferencedBy F2021L00313: ;
    rdfs:comment "5 37  Significant variations - Abrievated Graph Key: I129"@en-AU ;
    skos:definition "5 37  Significant variations"@en-AU ;
    skos:narrower F2021L00313:127 ;
    skos:prefLabel "Item I129"@en-AU ;
    dcat:accessURL <https://www.legislation.gov.au/F2021L00313/2023-08-04/2023-08-04/text/original/epub/OEBPS/document_1/document_1.html#_Toc144217974> ;
    dcat:landingPage "https://www.legislation.gov.au/F2021L00313/2023-08-04/2023-08-04/text/original/epub/OEBPS/document_1/document_1.html#_Toc144217974"^^xsd:anyURI ;
    dcat:theme legcons:Item .

F2021L00313:13 a legcons:Item,
        owl:Class,
        dcat:Resource ;
    rdfs:label "Item - I13 1 9  Modifications of certain terms used in the Australian Wild Game Meat Standard"@en-AU ;
    dct:isPartOf F2021L00313:1 ;
    dct:isReferencedBy F2021L00313: ;
    rdfs:comment "1 9  Modifications of certain terms used in the Australian Wild Game Meat Standard - Abrievated Graph Key: I13"@en-AU ;
    skos:definition "1 9  Modifications of certain terms used in the Australian Wild Game Meat Standard"@en-AU ;
    skos:narrower F2021L00313:1 ;
    skos:prefLabel "Item I13"@en-AU ;
    dcat:accessURL <https://www.legislation.gov.au/F2021L00313/2023-08-04/2023-08-04/text/original/epub/OEBPS/document_1/document_1.html#_Toc144217858> ;
    dcat:landingPage "https://www.legislation.gov.au/F2021L00313/2023-08-04/2023-08-04/text/original/epub/OEBPS/document_1/document_1.html#_Toc144217858"^^xsd:anyURI ;
    dcat:theme legcons:Item .

F2021L00313:131 a legcons:Item,
        owl:Class,
        dcat:Resource ;
    rdfs:label "Item - I131 5 38  Other reasons for requiring holder to vary approved arrangement"@en-AU ;
    dct:isPartOf F2021L00313:130 ;
    dct:isReferencedBy F2021L00313: ;
    rdfs:comment "5 38  Other reasons for requiring holder to vary approved arrangement - Abrievated Graph Key: I131"@en-AU ;
    skos:definition "5 38  Other reasons for requiring holder to vary approved arrangement"@en-AU ;
    skos:narrower F2021L00313:130 ;
    skos:prefLabel "Item I131"@en-AU ;
    dcat:accessURL <https://www.legislation.gov.au/F2021L00313/2023-08-04/2023-08-04/text/original/epub/OEBPS/document_1/document_1.html#_Toc144217976> ;
    dcat:landingPage "https://www.legislation.gov.au/F2021L00313/2023-08-04/2023-08-04/text/original/epub/OEBPS/document_1/document_1.html#_Toc144217976"^^xsd:anyURI ;
    dcat:theme legcons:Item .

F2021L00313:133 a legcons:Item,
        owl:Class,
        dcat:Resource ;
    rdfs:label "Item - I133 5 39  Application of this Part"@en-AU ;
    dct:isPartOf F2021L00313:132 ;
    dct:isReferencedBy F2021L00313: ;
    rdfs:comment "5 39  Application of this Part - Abrievated Graph Key: I133"@en-AU ;
    skos:definition "5 39  Application of this Part"@en-AU ;
    skos:narrower F2021L00313:132 ;
    skos:prefLabel "Item I133"@en-AU ;
    dcat:accessURL <https://www.legislation.gov.au/F2021L00313/2023-08-04/2023-08-04/text/original/epub/OEBPS/document_1/document_1.html#_Toc144217978> ;
    dcat:landingPage "https://www.legislation.gov.au/F2021L00313/2023-08-04/2023-08-04/text/original/epub/OEBPS/document_1/document_1.html#_Toc144217978"^^xsd:anyURI ;
    dcat:theme legcons:Item .

F2021L00313:134 a legcons:Item,
        owl:Class,
        dcat:Resource ;
    rdfs:label "Item - I134 5 40  Initial consideration period"@en-AU ;
    dct:isPartOf F2021L00313:132 ;
    dct:isReferencedBy F2021L00313: ;
    rdfs:comment "5 40  Initial consideration period - Abrievated Graph Key: I134"@en-AU ;
    skos:definition "5 40  Initial consideration period"@en-AU ;
    skos:narrower F2021L00313:132 ;
    skos:prefLabel "Item I134"@en-AU ;
    dcat:accessURL <https://www.legislation.gov.au/F2021L00313/2023-08-04/2023-08-04/text/original/epub/OEBPS/document_1/document_1.html#_Toc144217979> ;
    dcat:landingPage "https://www.legislation.gov.au/F2021L00313/2023-08-04/2023-08-04/text/original/epub/OEBPS/document_1/document_1.html#_Toc144217979"^^xsd:anyURI ;
    dcat:theme legcons:Item .

F2021L00313:135 a legcons:Item,
        owl:Class,
        dcat:Resource ;
    rdfs:label "Item - I135 5 41  Period within which request relating to application must be complied with"@en-AU ;
    dct:isPartOf F2021L00313:132 ;
    dct:isReferencedBy F2021L00313: ;
    rdfs:comment "5 41  Period within which request relating to application must be complied with - Abrievated Graph Key: I135"@en-AU ;
    skos:definition "5 41  Period within which request relating to application must be complied with"@en-AU ;
    skos:narrower F2021L00313:132 ;
    skos:prefLabel "Item I135"@en-AU ;
    dcat:accessURL <https://www.legislation.gov.au/F2021L00313/2023-08-04/2023-08-04/text/original/epub/OEBPS/document_1/document_1.html#_Toc144217980> ;
    dcat:landingPage "https://www.legislation.gov.au/F2021L00313/2023-08-04/2023-08-04/text/original/epub/OEBPS/document_1/document_1.html#_Toc144217980"^^xsd:anyURI ;
    dcat:theme legcons:Item .

F2021L00313:138 a legcons:Item,
        owl:Class,
        dcat:Resource ;
    rdfs:label "Item - I138 7 1  Period of effect of export permit"@en-AU ;
    dct:isPartOf F2021L00313:137 ;
    dct:isReferencedBy F2021L00313: ;
    rdfs:comment "7 1  Period of effect of export permit - Abrievated Graph Key: I138"@en-AU ;
    skos:definition "7 1  Period of effect of export permit"@en-AU ;
    skos:narrower F2021L00313:137 ;
    skos:prefLabel "Item I138"@en-AU ;
    dcat:accessURL <https://www.legislation.gov.au/F2021L00313/2023-08-04/2023-08-04/text/original/epub/OEBPS/document_1/document_1.html#_Toc144217983> ;
    dcat:landingPage "https://www.legislation.gov.au/F2021L00313/2023-08-04/2023-08-04/text/original/epub/OEBPS/document_1/document_1.html#_Toc144217983"^^xsd:anyURI ;
    dcat:theme legcons:Item .

F2021L00313:14 a legcons:Item,
        owl:Class,
        dcat:Resource ;
    rdfs:label "Item - I14 1 10  Circumstances in which alternative procedure standard or other requirement is taken to meet requirements of Australian Meat Standard or Australian Wild Game Meat Standard"@en-AU ;
    dct:isPartOf F2021L00313:1 ;
    dct:isReferencedBy F2021L00313: ;
    rdfs:comment "1 10  Circumstances in which alternative procedure standard or other requirement is taken to meet requirements of Australian Meat Standard or Australian Wild Game Meat Standard - Abrievated Graph Key: I14"@en-AU ;
    skos:definition "1 10  Circumstances in which alternative procedure standard or other requirement is taken to meet requirements of Australian Meat Standard or Australian Wild Game Meat Standard"@en-AU ;
    skos:narrower F2021L00313:1 ;
    skos:prefLabel "Item I14"@en-AU ;
    dcat:accessURL <https://www.legislation.gov.au/F2021L00313/2023-08-04/2023-08-04/text/original/epub/OEBPS/document_1/document_1.html#_Toc144217859> ;
    dcat:landingPage "https://www.legislation.gov.au/F2021L00313/2023-08-04/2023-08-04/text/original/epub/OEBPS/document_1/document_1.html#_Toc144217859"^^xsd:anyURI ;
    dcat:theme legcons:Item .

F2021L00313:140 a legcons:Item,
        owl:Class,
        dcat:Resource ;
    rdfs:label "Item - I140 7 2  Period of effect of varied export permit"@en-AU ;
    dct:isPartOf F2021L00313:139 ;
    dct:isReferencedBy F2021L00313: ;
    rdfs:comment "7 2  Period of effect of varied export permit - Abrievated Graph Key: I140"@en-AU ;
    skos:definition "7 2  Period of effect of varied export permit"@en-AU ;
    skos:narrower F2021L00313:139 ;
    skos:prefLabel "Item I140"@en-AU ;
    dcat:accessURL <https://www.legislation.gov.au/F2021L00313/2023-08-04/2023-08-04/text/original/epub/OEBPS/document_1/document_1.html#_Toc144217985> ;
    dcat:landingPage "https://www.legislation.gov.au/F2021L00313/2023-08-04/2023-08-04/text/original/epub/OEBPS/document_1/document_1.html#_Toc144217985"^^xsd:anyURI ;
    dcat:theme legcons:Item .

F2021L00313:141 a legcons:Item,
        owl:Class,
        dcat:Resource ;
    rdfs:label "Item - I141 7 3  Circumstances in which export permit may be suspended"@en-AU ;
    dct:isPartOf F2021L00313:139 ;
    dct:isReferencedBy F2021L00313: ;
    rdfs:comment "7 3  Circumstances in which export permit may be suspended - Abrievated Graph Key: I141"@en-AU ;
    skos:definition "7 3  Circumstances in which export permit may be suspended"@en-AU ;
    skos:narrower F2021L00313:139 ;
    skos:prefLabel "Item I141"@en-AU ;
    dcat:accessURL <https://www.legislation.gov.au/F2021L00313/2023-08-04/2023-08-04/text/original/epub/OEBPS/document_1/document_1.html#_Toc144217986> ;
    dcat:landingPage "https://www.legislation.gov.au/F2021L00313/2023-08-04/2023-08-04/text/original/epub/OEBPS/document_1/document_1.html#_Toc144217986"^^xsd:anyURI ;
    dcat:theme legcons:Item .

F2021L00313:142 a legcons:Item,
        owl:Class,
        dcat:Resource ;
    rdfs:label "Item - I142 7 4  Other circumstances in which export permit may be revoked"@en-AU ;
    dct:isPartOf F2021L00313:139 ;
    dct:isReferencedBy F2021L00313: ;
    rdfs:comment "7 4  Other circumstances in which export permit may be revoked - Abrievated Graph Key: I142"@en-AU ;
    skos:definition "7 4  Other circumstances in which export permit may be revoked"@en-AU ;
    skos:narrower F2021L00313:139 ;
    skos:prefLabel "Item I142"@en-AU ;
    dcat:accessURL <https://www.legislation.gov.au/F2021L00313/2023-08-04/2023-08-04/text/original/epub/OEBPS/document_1/document_1.html#_Toc144217987> ;
    dcat:landingPage "https://www.legislation.gov.au/F2021L00313/2023-08-04/2023-08-04/text/original/epub/OEBPS/document_1/document_1.html#_Toc144217987"^^xsd:anyURI ;
    dcat:theme legcons:Item .

F2021L00313:144 a legcons:Item,
        owl:Class,
        dcat:Resource ;
    rdfs:label "Item - I144 7 5  Changes that require additional or corrected information to be given to the Secretary"@en-AU ;
    dct:isPartOf F2021L00313:143 ;
    dct:isReferencedBy F2021L00313: ;
    rdfs:comment "7 5  Changes that require additional or corrected information to be given to the Secretary - Abrievated Graph Key: I144"@en-AU ;
    skos:definition "7 5  Changes that require additional or corrected information to be given to the Secretary"@en-AU ;
    skos:narrower F2021L00313:143 ;
    skos:prefLabel "Item I144"@en-AU ;
    dcat:accessURL <https://www.legislation.gov.au/F2021L00313/2023-08-04/2023-08-04/text/original/epub/OEBPS/document_1/document_1.html#_Toc144217989> ;
    dcat:landingPage "https://www.legislation.gov.au/F2021L00313/2023-08-04/2023-08-04/text/original/epub/OEBPS/document_1/document_1.html#_Toc144217989"^^xsd:anyURI ;
    dcat:theme legcons:Item .

F2021L00313:145 a legcons:Item,
        owl:Class,
        dcat:Resource ;
    rdfs:label "Item - I145 7 6  Return of export permit"@en-AU ;
    dct:isPartOf F2021L00313:143 ;
    dct:isReferencedBy F2021L00313: ;
    rdfs:comment "7 6  Return of export permit - Abrievated Graph Key: I145"@en-AU ;
    skos:definition "7 6  Return of export permit"@en-AU ;
    skos:narrower F2021L00313:143 ;
    skos:prefLabel "Item I145"@en-AU ;
    dcat:accessURL <https://www.legislation.gov.au/F2021L00313/2023-08-04/2023-08-04/text/original/epub/OEBPS/document_1/document_1.html#_Toc144217990> ;
    dcat:landingPage "https://www.legislation.gov.au/F2021L00313/2023-08-04/2023-08-04/text/original/epub/OEBPS/document_1/document_1.html#_Toc144217990"^^xsd:anyURI ;
    dcat:theme legcons:Item .

F2021L00313:146 a legcons:Item,
        owl:Class,
        dcat:Resource ;
    rdfs:label "Item - I146 7 7  Notification that prescribed wild game meat or wild game meat products are not to be exported"@en-AU ;
    dct:isPartOf F2021L00313:143 ;
    dct:isReferencedBy F2021L00313: ;
    rdfs:comment "7 7  Notification that prescribed wild game meat or wild game meat products are not to be exported - Abrievated Graph Key: I146"@en-AU ;
    skos:definition "7 7  Notification that prescribed wild game meat or wild game meat products are not to be exported"@en-AU ;
    skos:narrower F2021L00313:143 ;
    skos:prefLabel "Item I146"@en-AU ;
    dcat:accessURL <https://www.legislation.gov.au/F2021L00313/2023-08-04/2023-08-04/text/original/epub/OEBPS/document_1/document_1.html#_Toc144217991> ;
    dcat:landingPage "https://www.legislation.gov.au/F2021L00313/2023-08-04/2023-08-04/text/original/epub/OEBPS/document_1/document_1.html#_Toc144217991"^^xsd:anyURI ;
    dcat:theme legcons:Item .

F2021L00313:147 a legcons:Item,
        owl:Class,
        dcat:Resource ;
    rdfs:label "Item - I147 7 8  Application for export permit must include declaration"@en-AU ;
    dct:isPartOf F2021L00313:143 ;
    dct:isReferencedBy F2021L00313: ;
    rdfs:comment "7 8  Application for export permit must include declaration - Abrievated Graph Key: I147"@en-AU ;
    skos:definition "7 8  Application for export permit must include declaration"@en-AU ;
    skos:narrower F2021L00313:143 ;
    skos:prefLabel "Item I147"@en-AU ;
    dcat:accessURL <https://www.legislation.gov.au/F2021L00313/2023-08-04/2023-08-04/text/original/epub/OEBPS/document_1/document_1.html#_Toc144217992> ;
    dcat:landingPage "https://www.legislation.gov.au/F2021L00313/2023-08-04/2023-08-04/text/original/epub/OEBPS/document_1/document_1.html#_Toc144217992"^^xsd:anyURI ;
    dcat:theme legcons:Item .

F2021L00313:150 a legcons:Item,
        owl:Class,
        dcat:Resource ;
    rdfs:label "Item - I150 8 1  Information to be included in notice of intention to export"@en-AU ;
    dct:isPartOf F2021L00313:149 ;
    dct:isReferencedBy F2021L00313: ;
    rdfs:comment "8 1  Information to be included in notice of intention to export - Abrievated Graph Key: I150"@en-AU ;
    skos:definition "8 1  Information to be included in notice of intention to export"@en-AU ;
    skos:narrower F2021L00313:149 ;
    skos:prefLabel "Item I150"@en-AU ;
    dcat:accessURL <https://www.legislation.gov.au/F2021L00313/2023-08-04/2023-08-04/text/original/epub/OEBPS/document_1/document_1.html#_Toc144217995> ;
    dcat:landingPage "https://www.legislation.gov.au/F2021L00313/2023-08-04/2023-08-04/text/original/epub/OEBPS/document_1/document_1.html#_Toc144217995"^^xsd:anyURI ;
    dcat:theme legcons:Item .

F2021L00313:151 a legcons:Item,
        owl:Class,
        dcat:Resource ;
    rdfs:label "Item - I151 8 2  Person who must give notice of intention to export"@en-AU ;
    dct:isPartOf F2021L00313:149 ;
    dct:isReferencedBy F2021L00313: ;
    rdfs:comment "8 2  Person who must give notice of intention to export - Abrievated Graph Key: I151"@en-AU ;
    skos:definition "8 2  Person who must give notice of intention to export"@en-AU ;
    skos:narrower F2021L00313:149 ;
    skos:prefLabel "Item I151"@en-AU ;
    dcat:accessURL <https://www.legislation.gov.au/F2021L00313/2023-08-04/2023-08-04/text/original/epub/OEBPS/document_1/document_1.html#_Toc144217996> ;
    dcat:landingPage "https://www.legislation.gov.au/F2021L00313/2023-08-04/2023-08-04/text/original/epub/OEBPS/document_1/document_1.html#_Toc144217996"^^xsd:anyURI ;
    dcat:theme legcons:Item .

F2021L00313:152 a legcons:Item,
        owl:Class,
        dcat:Resource ;
    rdfs:label "Item - I152 8 3  Person to whom notice of intention to export must be given"@en-AU ;
    dct:isPartOf F2021L00313:149 ;
    dct:isReferencedBy F2021L00313: ;
    rdfs:comment "8 3  Person to whom notice of intention to export must be given - Abrievated Graph Key: I152"@en-AU ;
    skos:definition "8 3  Person to whom notice of intention to export must be given"@en-AU ;
    skos:narrower F2021L00313:149 ;
    skos:prefLabel "Item I152"@en-AU ;
    dcat:accessURL <https://www.legislation.gov.au/F2021L00313/2023-08-04/2023-08-04/text/original/epub/OEBPS/document_1/document_1.html#_Toc144217997> ;
    dcat:landingPage "https://www.legislation.gov.au/F2021L00313/2023-08-04/2023-08-04/text/original/epub/OEBPS/document_1/document_1.html#_Toc144217997"^^xsd:anyURI ;
    dcat:theme legcons:Item .

F2021L00313:153 a legcons:Item,
        owl:Class,
        dcat:Resource ;
    rdfs:label "Item - I153 8 4  When notice of intention to export must be given"@en-AU ;
    dct:isPartOf F2021L00313:149 ;
    dct:isReferencedBy F2021L00313: ;
    rdfs:comment "8 4  When notice of intention to export must be given - Abrievated Graph Key: I153"@en-AU ;
    skos:definition "8 4  When notice of intention to export must be given"@en-AU ;
    skos:narrower F2021L00313:149 ;
    skos:prefLabel "Item I153"@en-AU ;
    dcat:accessURL <https://www.legislation.gov.au/F2021L00313/2023-08-04/2023-08-04/text/original/epub/OEBPS/document_1/document_1.html#_Toc144217998> ;
    dcat:landingPage "https://www.legislation.gov.au/F2021L00313/2023-08-04/2023-08-04/text/original/epub/OEBPS/document_1/document_1.html#_Toc144217998"^^xsd:anyURI ;
    dcat:theme legcons:Item .

F2021L00313:155 a legcons:Item,
        owl:Class,
        dcat:Resource ;
    rdfs:label "Item - I155 8 5  Purpose of this Part"@en-AU ;
    dct:isPartOf F2021L00313:154 ;
    dct:isReferencedBy F2021L00313: ;
    rdfs:comment "8 5  Purpose of this Part - Abrievated Graph Key: I155"@en-AU ;
    skos:definition "8 5  Purpose of this Part"@en-AU ;
    skos:narrower F2021L00313:154 ;
    skos:prefLabel "Item I155"@en-AU ;
    dcat:accessURL <https://www.legislation.gov.au/F2021L00313/2023-08-04/2023-08-04/text/original/epub/OEBPS/document_1/document_1.html#_Toc144218000> ;
    dcat:landingPage "https://www.legislation.gov.au/F2021L00313/2023-08-04/2023-08-04/text/original/epub/OEBPS/document_1/document_1.html#_Toc144218000"^^xsd:anyURI ;
    dcat:theme legcons:Item .

F2021L00313:156 a legcons:Item,
        owl:Class,
        dcat:Resource ;
    rdfs:label "Item - I156 8 6  General requirements for trade descriptions"@en-AU ;
    dct:isPartOf F2021L00313:154 ;
    dct:isReferencedBy F2021L00313: ;
    rdfs:comment "8 6  General requirements for trade descriptions - Abrievated Graph Key: I156"@en-AU ;
    skos:definition "8 6  General requirements for trade descriptions"@en-AU ;
    skos:narrower F2021L00313:154 ;
    skos:prefLabel "Item I156"@en-AU ;
    dcat:accessURL <https://www.legislation.gov.au/F2021L00313/2023-08-04/2023-08-04/text/original/epub/OEBPS/document_1/document_1.html#_Toc144218001> ;
    dcat:landingPage "https://www.legislation.gov.au/F2021L00313/2023-08-04/2023-08-04/text/original/epub/OEBPS/document_1/document_1.html#_Toc144218001"^^xsd:anyURI ;
    dcat:theme legcons:Item .

F2021L00313:157 a legcons:Item,
        owl:Class,
        dcat:Resource ;
    rdfs:label "Item - I157 8 7  Trade descriptions in language other than English"@en-AU ;
    dct:isPartOf F2021L00313:154 ;
    dct:isReferencedBy F2021L00313: ;
    rdfs:comment "8 7  Trade descriptions in language other than English - Abrievated Graph Key: I157"@en-AU ;
    skos:definition "8 7  Trade descriptions in language other than English"@en-AU ;
    skos:narrower F2021L00313:154 ;
    skos:prefLabel "Item I157"@en-AU ;
    dcat:accessURL <https://www.legislation.gov.au/F2021L00313/2023-08-04/2023-08-04/text/original/epub/OEBPS/document_1/document_1.html#_Toc144218002> ;
    dcat:landingPage "https://www.legislation.gov.au/F2021L00313/2023-08-04/2023-08-04/text/original/epub/OEBPS/document_1/document_1.html#_Toc144218002"^^xsd:anyURI ;
    dcat:theme legcons:Item .

F2021L00313:160 a legcons:Item,
        owl:Class,
        dcat:Resource ;
    rdfs:label "Item - I160 8 8  Purpose of this Division"@en-AU ;
    dct:isPartOf F2021L00313:159 ;
    dct:isReferencedBy F2021L00313: ;
    rdfs:comment "8 8  Purpose of this Division - Abrievated Graph Key: I160"@en-AU ;
    skos:definition "8 8  Purpose of this Division"@en-AU ;
    skos:narrower F2021L00313:159 ;
    skos:prefLabel "Item I160"@en-AU ;
    dcat:accessURL <https://www.legislation.gov.au/F2021L00313/2023-08-04/2023-08-04/text/original/epub/OEBPS/document_1/document_1.html#_Toc144218005> ;
    dcat:landingPage "https://www.legislation.gov.au/F2021L00313/2023-08-04/2023-08-04/text/original/epub/OEBPS/document_1/document_1.html#_Toc144218005"^^xsd:anyURI ;
    dcat:theme legcons:Item .

F2021L00313:161 a legcons:Item,
        owl:Class,
        dcat:Resource ;
    rdfs:label "Item - I161 8 9  Tolerances for dimensions of official marks"@en-AU ;
    dct:isPartOf F2021L00313:159 ;
    dct:isReferencedBy F2021L00313: ;
    rdfs:comment "8 9  Tolerances for dimensions of official marks - Abrievated Graph Key: I161"@en-AU ;
    skos:definition "8 9  Tolerances for dimensions of official marks"@en-AU ;
    skos:narrower F2021L00313:159 ;
    skos:prefLabel "Item I161"@en-AU ;
    dcat:accessURL <https://www.legislation.gov.au/F2021L00313/2023-08-04/2023-08-04/text/original/epub/OEBPS/document_1/document_1.html#_Toc144218006> ;
    dcat:landingPage "https://www.legislation.gov.au/F2021L00313/2023-08-04/2023-08-04/text/original/epub/OEBPS/document_1/document_1.html#_Toc144218006"^^xsd:anyURI ;
    dcat:theme legcons:Item .

F2021L00313:162 a legcons:Item,
        owl:Class,
        dcat:Resource ;
    rdfs:label "Item - I162 8 10  Official markAustralia Approved"@en-AU ;
    dct:isPartOf F2021L00313:159 ;
    dct:isReferencedBy F2021L00313: ;
    rdfs:comment "8 10  Official markAustralia Approved - Abrievated Graph Key: I162"@en-AU ;
    skos:definition "8 10  Official markAustralia Approved"@en-AU ;
    skos:narrower F2021L00313:159 ;
    skos:prefLabel "Item I162"@en-AU ;
    dcat:accessURL <https://www.legislation.gov.au/F2021L00313/2023-08-04/2023-08-04/text/original/epub/OEBPS/document_1/document_1.html#_Toc144218007> ;
    dcat:landingPage "https://www.legislation.gov.au/F2021L00313/2023-08-04/2023-08-04/text/original/epub/OEBPS/document_1/document_1.html#_Toc144218007"^^xsd:anyURI ;
    dcat:theme legcons:Item .

F2021L00313:163 a legcons:Item,
        owl:Class,
        dcat:Resource ;
    rdfs:label "Item - I163 8 11  Official markforeign country identification"@en-AU ;
    dct:isPartOf F2021L00313:159 ;
    dct:isReferencedBy F2021L00313: ;
    rdfs:comment "8 11  Official markforeign country identification - Abrievated Graph Key: I163"@en-AU ;
    skos:definition "8 11  Official markforeign country identification"@en-AU ;
    skos:narrower F2021L00313:159 ;
    skos:prefLabel "Item I163"@en-AU ;
    dcat:accessURL <https://www.legislation.gov.au/F2021L00313/2023-08-04/2023-08-04/text/original/epub/OEBPS/document_1/document_1.html#_Toc144218008> ;
    dcat:landingPage "https://www.legislation.gov.au/F2021L00313/2023-08-04/2023-08-04/text/original/epub/OEBPS/document_1/document_1.html#_Toc144218008"^^xsd:anyURI ;
    dcat:theme legcons:Item .

F2021L00313:164 a legcons:Item,
        owl:Class,
        dcat:Resource ;
    rdfs:label "Item - I164 8 12  Official marktamper indicative metal strap seal"@en-AU ;
    dct:isPartOf F2021L00313:159 ;
    dct:isReferencedBy F2021L00313: ;
    rdfs:comment "8 12  Official marktamper indicative metal strap seal - Abrievated Graph Key: I164"@en-AU ;
    skos:definition "8 12  Official marktamper indicative metal strap seal"@en-AU ;
    skos:narrower F2021L00313:159 ;
    skos:prefLabel "Item I164"@en-AU ;
    dcat:accessURL <https://www.legislation.gov.au/F2021L00313/2023-08-04/2023-08-04/text/original/epub/OEBPS/document_1/document_1.html#_Toc144218009> ;
    dcat:landingPage "https://www.legislation.gov.au/F2021L00313/2023-08-04/2023-08-04/text/original/epub/OEBPS/document_1/document_1.html#_Toc144218009"^^xsd:anyURI ;
    dcat:theme legcons:Item .

F2021L00313:165 a legcons:Item,
        owl:Class,
        dcat:Resource ;
    rdfs:label "Item - I165 8 13  Official markbolt seal"@en-AU ;
    dct:isPartOf F2021L00313:159 ;
    dct:isReferencedBy F2021L00313: ;
    rdfs:comment "8 13  Official markbolt seal - Abrievated Graph Key: I165"@en-AU ;
    skos:definition "8 13  Official markbolt seal"@en-AU ;
    skos:narrower F2021L00313:159 ;
    skos:prefLabel "Item I165"@en-AU ;
    dcat:accessURL <https://www.legislation.gov.au/F2021L00313/2023-08-04/2023-08-04/text/original/epub/OEBPS/document_1/document_1.html#_Toc144218010> ;
    dcat:landingPage "https://www.legislation.gov.au/F2021L00313/2023-08-04/2023-08-04/text/original/epub/OEBPS/document_1/document_1.html#_Toc144218010"^^xsd:anyURI ;
    dcat:theme legcons:Item .

F2021L00313:166 a legcons:Item,
        owl:Class,
        dcat:Resource ;
    rdfs:label "Item - I166 8 14  Official markApproved for Export"@en-AU ;
    dct:isPartOf F2021L00313:159 ;
    dct:isReferencedBy F2021L00313: ;
    rdfs:comment "8 14  Official markApproved for Export - Abrievated Graph Key: I166"@en-AU ;
    skos:definition "8 14  Official markApproved for Export"@en-AU ;
    skos:narrower F2021L00313:159 ;
    skos:prefLabel "Item I166"@en-AU ;
    dcat:accessURL <https://www.legislation.gov.au/F2021L00313/2023-08-04/2023-08-04/text/original/epub/OEBPS/document_1/document_1.html#_Toc144218011> ;
    dcat:landingPage "https://www.legislation.gov.au/F2021L00313/2023-08-04/2023-08-04/text/original/epub/OEBPS/document_1/document_1.html#_Toc144218011"^^xsd:anyURI ;
    dcat:theme legcons:Item .

F2021L00313:167 a legcons:Item,
        owl:Class,
        dcat:Resource ;
    rdfs:label "Item - I167 8 15  Official markEuropean Union"@en-AU ;
    dct:isPartOf F2021L00313:159 ;
    dct:isReferencedBy F2021L00313: ;
    rdfs:comment "8 15  Official markEuropean Union - Abrievated Graph Key: I167"@en-AU ;
    skos:definition "8 15  Official markEuropean Union"@en-AU ;
    skos:narrower F2021L00313:159 ;
    skos:prefLabel "Item I167"@en-AU ;
    dcat:accessURL <https://www.legislation.gov.au/F2021L00313/2023-08-04/2023-08-04/text/original/epub/OEBPS/document_1/document_1.html#_Toc144218012> ;
    dcat:landingPage "https://www.legislation.gov.au/F2021L00313/2023-08-04/2023-08-04/text/original/epub/OEBPS/document_1/document_1.html#_Toc144218012"^^xsd:anyURI ;
    dcat:theme legcons:Item .

F2021L00313:168 a legcons:Item,
        owl:Class,
        dcat:Resource ;
    rdfs:label "Item - I168 8 16  Official markcarton seal"@en-AU ;
    dct:isPartOf F2021L00313:159 ;
    dct:isReferencedBy F2021L00313: ;
    rdfs:comment "8 16  Official markcarton seal - Abrievated Graph Key: I168"@en-AU ;
    skos:definition "8 16  Official markcarton seal"@en-AU ;
    skos:narrower F2021L00313:159 ;
    skos:prefLabel "Item I168"@en-AU ;
    dcat:accessURL <https://www.legislation.gov.au/F2021L00313/2023-08-04/2023-08-04/text/original/epub/OEBPS/document_1/document_1.html#_Toc144218013> ;
    dcat:landingPage "https://www.legislation.gov.au/F2021L00313/2023-08-04/2023-08-04/text/original/epub/OEBPS/document_1/document_1.html#_Toc144218013"^^xsd:anyURI ;
    dcat:theme legcons:Item .

F2021L00313:169 a legcons:Item,
        owl:Class,
        dcat:Resource ;
    rdfs:label "Item - I169 8 17  Official markwild game meat or wild game meat products opened for assessment and resealed"@en-AU ;
    dct:isPartOf F2021L00313:159 ;
    dct:isReferencedBy F2021L00313: ;
    rdfs:comment "8 17  Official markwild game meat or wild game meat products opened for assessment and resealed - Abrievated Graph Key: I169"@en-AU ;
    skos:definition "8 17  Official markwild game meat or wild game meat products opened for assessment and resealed"@en-AU ;
    skos:narrower F2021L00313:159 ;
    skos:prefLabel "Item I169"@en-AU ;
    dcat:accessURL <https://www.legislation.gov.au/F2021L00313/2023-08-04/2023-08-04/text/original/epub/OEBPS/document_1/document_1.html#_Toc144218014> ;
    dcat:landingPage "https://www.legislation.gov.au/F2021L00313/2023-08-04/2023-08-04/text/original/epub/OEBPS/document_1/document_1.html#_Toc144218014"^^xsd:anyURI ;
    dcat:theme legcons:Item .

F2021L00313:170 a legcons:Item,
        owl:Class,
        dcat:Resource ;
    rdfs:label "Item - I170 8 18  Official markAustralian Government"@en-AU ;
    dct:isPartOf F2021L00313:159 ;
    dct:isReferencedBy F2021L00313: ;
    rdfs:comment "8 18  Official markAustralian Government - Abrievated Graph Key: I170"@en-AU ;
    skos:definition "8 18  Official markAustralian Government"@en-AU ;
    skos:narrower F2021L00313:159 ;
    skos:prefLabel "Item I170"@en-AU ;
    dcat:accessURL <https://www.legislation.gov.au/F2021L00313/2023-08-04/2023-08-04/text/original/epub/OEBPS/document_1/document_1.html#_Toc144218015> ;
    dcat:landingPage "https://www.legislation.gov.au/F2021L00313/2023-08-04/2023-08-04/text/original/epub/OEBPS/document_1/document_1.html#_Toc144218015"^^xsd:anyURI ;
    dcat:theme legcons:Item .

F2021L00313:172 a legcons:Item,
        owl:Class,
        dcat:Resource ;
    rdfs:label "Item - I172 8 19  Purpose and application of this Division"@en-AU ;
    dct:isPartOf F2021L00313:171 ;
    dct:isReferencedBy F2021L00313: ;
    rdfs:comment "8 19  Purpose and application of this Division - Abrievated Graph Key: I172"@en-AU ;
    skos:definition "8 19  Purpose and application of this Division"@en-AU ;
    skos:narrower F2021L00313:171 ;
    skos:prefLabel "Item I172"@en-AU ;
    dcat:accessURL <https://www.legislation.gov.au/F2021L00313/2023-08-04/2023-08-04/text/original/epub/OEBPS/document_1/document_1.html#_Toc144218017> ;
    dcat:landingPage "https://www.legislation.gov.au/F2021L00313/2023-08-04/2023-08-04/text/original/epub/OEBPS/document_1/document_1.html#_Toc144218017"^^xsd:anyURI ;
    dcat:theme legcons:Item .

F2021L00313:173 a legcons:Item,
        owl:Class,
        dcat:Resource ;
    rdfs:label "Item - I173 8 20  Interpretation"@en-AU ;
    dct:isPartOf F2021L00313:171 ;
    dct:isReferencedBy F2021L00313: ;
    rdfs:comment "8 20  Interpretation - Abrievated Graph Key: I173"@en-AU ;
    skos:definition "8 20  Interpretation"@en-AU ;
    skos:narrower F2021L00313:171 ;
    skos:prefLabel "Item I173"@en-AU ;
    dcat:accessURL <https://www.legislation.gov.au/F2021L00313/2023-08-04/2023-08-04/text/original/epub/OEBPS/document_1/document_1.html#_Toc144218018> ;
    dcat:landingPage "https://www.legislation.gov.au/F2021L00313/2023-08-04/2023-08-04/text/original/epub/OEBPS/document_1/document_1.html#_Toc144218018"^^xsd:anyURI ;
    dcat:theme legcons:Item .

F2021L00313:174 a legcons:Item,
        owl:Class,
        dcat:Resource ;
    rdfs:label "Item - I174 8 21  Persons who may manufacture or supply official marks for wild game meat or wild game meat products"@en-AU ;
    dct:isPartOf F2021L00313:171 ;
    dct:isReferencedBy F2021L00313: ;
    rdfs:comment "8 21  Persons who may manufacture or supply official marks for wild game meat or wild game meat products - Abrievated Graph Key: I174"@en-AU ;
    skos:definition "8 21  Persons who may manufacture or supply official marks for wild game meat or wild game meat products"@en-AU ;
    skos:narrower F2021L00313:171 ;
    skos:prefLabel "Item I174"@en-AU ;
    dcat:accessURL <https://www.legislation.gov.au/F2021L00313/2023-08-04/2023-08-04/text/original/epub/OEBPS/document_1/document_1.html#_Toc144218019> ;
    dcat:landingPage "https://www.legislation.gov.au/F2021L00313/2023-08-04/2023-08-04/text/original/epub/OEBPS/document_1/document_1.html#_Toc144218019"^^xsd:anyURI ;
    dcat:theme legcons:Item .

F2021L00313:175 a legcons:Item,
        owl:Class,
        dcat:Resource ;
    rdfs:label "Item - I175 8 22  Persons who may possess official marks that have not been applied to wild game meat or wild game meat products"@en-AU ;
    dct:isPartOf F2021L00313:171 ;
    dct:isReferencedBy F2021L00313: ;
    rdfs:comment "8 22  Persons who may possess official marks that have not been applied to wild game meat or wild game meat products - Abrievated Graph Key: I175"@en-AU ;
    skos:definition "8 22  Persons who may possess official marks that have not been applied to wild game meat or wild game meat products"@en-AU ;
    skos:narrower F2021L00313:171 ;
    skos:prefLabel "Item I175"@en-AU ;
    dcat:accessURL <https://www.legislation.gov.au/F2021L00313/2023-08-04/2023-08-04/text/original/epub/OEBPS/document_1/document_1.html#_Toc144218020> ;
    dcat:landingPage "https://www.legislation.gov.au/F2021L00313/2023-08-04/2023-08-04/text/original/epub/OEBPS/document_1/document_1.html#_Toc144218020"^^xsd:anyURI ;
    dcat:theme legcons:Item .

F2021L00313:176 a legcons:Item,
        owl:Class,
        dcat:Resource ;
    rdfs:label "Item - I176 8 23  Persons who may apply official marks to wild game meat or wild game meat products etc"@en-AU ;
    dct:isPartOf F2021L00313:171 ;
    dct:isReferencedBy F2021L00313: ;
    rdfs:comment "8 23  Persons who may apply official marks to wild game meat or wild game meat products etc - Abrievated Graph Key: I176"@en-AU ;
    skos:definition "8 23  Persons who may apply official marks to wild game meat or wild game meat products etc"@en-AU ;
    skos:narrower F2021L00313:171 ;
    skos:prefLabel "Item I176"@en-AU ;
    dcat:accessURL <https://www.legislation.gov.au/F2021L00313/2023-08-04/2023-08-04/text/original/epub/OEBPS/document_1/document_1.html#_Toc144218021> ;
    dcat:landingPage "https://www.legislation.gov.au/F2021L00313/2023-08-04/2023-08-04/text/original/epub/OEBPS/document_1/document_1.html#_Toc144218021"^^xsd:anyURI ;
    dcat:theme legcons:Item .

F2021L00313:177 a legcons:Item,
        owl:Class,
        dcat:Resource ;
    rdfs:label "Item - I177 8 24  Circumstances in which official mark must not be applied to wild game meat or wild game meat products"@en-AU ;
    dct:isPartOf F2021L00313:171 ;
    dct:isReferencedBy F2021L00313: ;
    rdfs:comment "8 24  Circumstances in which official mark must not be applied to wild game meat or wild game meat products - Abrievated Graph Key: I177"@en-AU ;
    skos:definition "8 24  Circumstances in which official mark must not be applied to wild game meat or wild game meat products"@en-AU ;
    skos:narrower F2021L00313:171 ;
    skos:prefLabel "Item I177"@en-AU ;
    dcat:accessURL <https://www.legislation.gov.au/F2021L00313/2023-08-04/2023-08-04/text/original/epub/OEBPS/document_1/document_1.html#_Toc144218022> ;
    dcat:landingPage "https://www.legislation.gov.au/F2021L00313/2023-08-04/2023-08-04/text/original/epub/OEBPS/document_1/document_1.html#_Toc144218022"^^xsd:anyURI ;
    dcat:theme legcons:Item .

F2021L00313:178 a legcons:Item,
        owl:Class,
        dcat:Resource ;
    rdfs:label "Item - I178 8 25  Alteration of and interference with official marks"@en-AU ;
    dct:isPartOf F2021L00313:171 ;
    dct:isReferencedBy F2021L00313: ;
    rdfs:comment "8 25  Alteration of and interference with official marks - Abrievated Graph Key: I178"@en-AU ;
    skos:definition "8 25  Alteration of and interference with official marks"@en-AU ;
    skos:narrower F2021L00313:171 ;
    skos:prefLabel "Item I178"@en-AU ;
    dcat:accessURL <https://www.legislation.gov.au/F2021L00313/2023-08-04/2023-08-04/text/original/epub/OEBPS/document_1/document_1.html#_Toc144218023> ;
    dcat:landingPage "https://www.legislation.gov.au/F2021L00313/2023-08-04/2023-08-04/text/original/epub/OEBPS/document_1/document_1.html#_Toc144218023"^^xsd:anyURI ;
    dcat:theme legcons:Item .

F2021L00313:179 a legcons:Item,
        owl:Class,
        dcat:Resource ;
    rdfs:label "Item - I179 8 26  Official marks must be legible and securely attached"@en-AU ;
    dct:isPartOf F2021L00313:171 ;
    dct:isReferencedBy F2021L00313: ;
    rdfs:comment "8 26  Official marks must be legible and securely attached - Abrievated Graph Key: I179"@en-AU ;
    skos:definition "8 26  Official marks must be legible and securely attached"@en-AU ;
    skos:narrower F2021L00313:171 ;
    skos:prefLabel "Item I179"@en-AU ;
    dcat:accessURL <https://www.legislation.gov.au/F2021L00313/2023-08-04/2023-08-04/text/original/epub/OEBPS/document_1/document_1.html#_Toc144218024> ;
    dcat:landingPage "https://www.legislation.gov.au/F2021L00313/2023-08-04/2023-08-04/text/original/epub/OEBPS/document_1/document_1.html#_Toc144218024"^^xsd:anyURI ;
    dcat:theme legcons:Item .

F2021L00313:18 a legcons:Item,
        owl:Class,
        dcat:Resource ;
    rdfs:label "Item - I18 2 1  Wild game meat and wild game meat products that are prescribed goods"@en-AU ;
    dct:isPartOf F2021L00313:17 ;
    dct:isReferencedBy F2021L00313: ;
    rdfs:comment "2 1  Wild game meat and wild game meat products that are prescribed goods - Abrievated Graph Key: I18"@en-AU ;
    skos:definition "2 1  Wild game meat and wild game meat products that are prescribed goods"@en-AU ;
    skos:narrower F2021L00313:17 ;
    skos:prefLabel "Item I18"@en-AU ;
    dcat:accessURL <https://www.legislation.gov.au/F2021L00313/2023-08-04/2023-08-04/text/original/epub/OEBPS/document_1/document_1.html#_Toc144217863> ;
    dcat:landingPage "https://www.legislation.gov.au/F2021L00313/2023-08-04/2023-08-04/text/original/epub/OEBPS/document_1/document_1.html#_Toc144217863"^^xsd:anyURI ;
    dcat:theme legcons:Item .

F2021L00313:180 a legcons:Item,
        owl:Class,
        dcat:Resource ;
    rdfs:label "Item - I180 8 27  Security of official marks"@en-AU ;
    dct:isPartOf F2021L00313:171 ;
    dct:isReferencedBy F2021L00313: ;
    rdfs:comment "8 27  Security of official marks - Abrievated Graph Key: I180"@en-AU ;
    skos:definition "8 27  Security of official marks"@en-AU ;
    skos:narrower F2021L00313:171 ;
    skos:prefLabel "Item I180"@en-AU ;
    dcat:accessURL <https://www.legislation.gov.au/F2021L00313/2023-08-04/2023-08-04/text/original/epub/OEBPS/document_1/document_1.html#_Toc144218025> ;
    dcat:landingPage "https://www.legislation.gov.au/F2021L00313/2023-08-04/2023-08-04/text/original/epub/OEBPS/document_1/document_1.html#_Toc144218025"^^xsd:anyURI ;
    dcat:theme legcons:Item .

F2021L00313:181 a legcons:Item,
        owl:Class,
        dcat:Resource ;
    rdfs:label "Item - I181 8 28  Removal or defacement of official marks"@en-AU ;
    dct:isPartOf F2021L00313:171 ;
    dct:isReferencedBy F2021L00313: ;
    rdfs:comment "8 28  Removal or defacement of official marks - Abrievated Graph Key: I181"@en-AU ;
    skos:definition "8 28  Removal or defacement of official marks"@en-AU ;
    skos:narrower F2021L00313:171 ;
    skos:prefLabel "Item I181"@en-AU ;
    dcat:accessURL <https://www.legislation.gov.au/F2021L00313/2023-08-04/2023-08-04/text/original/epub/OEBPS/document_1/document_1.html#_Toc144218026> ;
    dcat:landingPage "https://www.legislation.gov.au/F2021L00313/2023-08-04/2023-08-04/text/original/epub/OEBPS/document_1/document_1.html#_Toc144218026"^^xsd:anyURI ;
    dcat:theme legcons:Item .

F2021L00313:182 a legcons:Item,
        owl:Class,
        dcat:Resource ;
    rdfs:label "Item - I182 8 29  Records of official marks manufactured or supplied"@en-AU ;
    dct:isPartOf F2021L00313:171 ;
    dct:isReferencedBy F2021L00313: ;
    rdfs:comment "8 29  Records of official marks manufactured or supplied - Abrievated Graph Key: I182"@en-AU ;
    skos:definition "8 29  Records of official marks manufactured or supplied"@en-AU ;
    skos:narrower F2021L00313:171 ;
    skos:prefLabel "Item I182"@en-AU ;
    dcat:accessURL <https://www.legislation.gov.au/F2021L00313/2023-08-04/2023-08-04/text/original/epub/OEBPS/document_1/document_1.html#_Toc144218027> ;
    dcat:landingPage "https://www.legislation.gov.au/F2021L00313/2023-08-04/2023-08-04/text/original/epub/OEBPS/document_1/document_1.html#_Toc144218027"^^xsd:anyURI ;
    dcat:theme legcons:Item .

F2021L00313:183 a legcons:Item,
        owl:Class,
        dcat:Resource ;
    rdfs:label "Item - I183 8 30  Records of official marks received applied removed defaced destroyed or returned"@en-AU ;
    dct:isPartOf F2021L00313:171 ;
    dct:isReferencedBy F2021L00313: ;
    rdfs:comment "8 30  Records of official marks received applied removed defaced destroyed or returned - Abrievated Graph Key: I183"@en-AU ;
    skos:definition "8 30  Records of official marks received applied removed defaced destroyed or returned"@en-AU ;
    skos:narrower F2021L00313:171 ;
    skos:prefLabel "Item I183"@en-AU ;
    dcat:accessURL <https://www.legislation.gov.au/F2021L00313/2023-08-04/2023-08-04/text/original/epub/OEBPS/document_1/document_1.html#_Toc144218028> ;
    dcat:landingPage "https://www.legislation.gov.au/F2021L00313/2023-08-04/2023-08-04/text/original/epub/OEBPS/document_1/document_1.html#_Toc144218028"^^xsd:anyURI ;
    dcat:theme legcons:Item .

F2021L00313:185 a legcons:Item,
        owl:Class,
        dcat:Resource ;
    rdfs:label "Item - I185 8 31  Purpose of this Division"@en-AU ;
    dct:isPartOf F2021L00313:184 ;
    dct:isReferencedBy F2021L00313: ;
    rdfs:comment "8 31  Purpose of this Division - Abrievated Graph Key: I185"@en-AU ;
    skos:definition "8 31  Purpose of this Division"@en-AU ;
    skos:narrower F2021L00313:184 ;
    skos:prefLabel "Item I185"@en-AU ;
    dcat:accessURL <https://www.legislation.gov.au/F2021L00313/2023-08-04/2023-08-04/text/original/epub/OEBPS/document_1/document_1.html#_Toc144218030> ;
    dcat:landingPage "https://www.legislation.gov.au/F2021L00313/2023-08-04/2023-08-04/text/original/epub/OEBPS/document_1/document_1.html#_Toc144218030"^^xsd:anyURI ;
    dcat:theme legcons:Item .

F2021L00313:186 a legcons:Item,
        owl:Class,
        dcat:Resource ;
    rdfs:label "Item - I186 8 32  Circumstances in which a mark resembles an official mark"@en-AU ;
    dct:isPartOf F2021L00313:184 ;
    dct:isReferencedBy F2021L00313: ;
    rdfs:comment "8 32  Circumstances in which a mark resembles an official mark - Abrievated Graph Key: I186"@en-AU ;
    skos:definition "8 32  Circumstances in which a mark resembles an official mark"@en-AU ;
    skos:narrower F2021L00313:184 ;
    skos:prefLabel "Item I186"@en-AU ;
    dcat:accessURL <https://www.legislation.gov.au/F2021L00313/2023-08-04/2023-08-04/text/original/epub/OEBPS/document_1/document_1.html#_Toc144218031> ;
    dcat:landingPage "https://www.legislation.gov.au/F2021L00313/2023-08-04/2023-08-04/text/original/epub/OEBPS/document_1/document_1.html#_Toc144218031"^^xsd:anyURI ;
    dcat:theme legcons:Item .

F2021L00313:187 a legcons:Item,
        owl:Class,
        dcat:Resource ;
    rdfs:label "Item - I187 8 33  Persons who may apply a resemblance"@en-AU ;
    dct:isPartOf F2021L00313:184 ;
    dct:isReferencedBy F2021L00313: ;
    rdfs:comment "8 33  Persons who may apply a resemblance - Abrievated Graph Key: I187"@en-AU ;
    skos:definition "8 33  Persons who may apply a resemblance"@en-AU ;
    skos:narrower F2021L00313:184 ;
    skos:prefLabel "Item I187"@en-AU ;
    dcat:accessURL <https://www.legislation.gov.au/F2021L00313/2023-08-04/2023-08-04/text/original/epub/OEBPS/document_1/document_1.html#_Toc144218032> ;
    dcat:landingPage "https://www.legislation.gov.au/F2021L00313/2023-08-04/2023-08-04/text/original/epub/OEBPS/document_1/document_1.html#_Toc144218032"^^xsd:anyURI ;
    dcat:theme legcons:Item .

F2021L00313:189 a legcons:Item,
        owl:Class,
        dcat:Resource ;
    rdfs:label "Item - I189 8 34  Purpose of this Division"@en-AU ;
    dct:isPartOf F2021L00313:188 ;
    dct:isReferencedBy F2021L00313: ;
    rdfs:comment "8 34  Purpose of this Division - Abrievated Graph Key: I189"@en-AU ;
    skos:definition "8 34  Purpose of this Division"@en-AU ;
    skos:narrower F2021L00313:188 ;
    skos:prefLabel "Item I189"@en-AU ;
    dcat:accessURL <https://www.legislation.gov.au/F2021L00313/2023-08-04/2023-08-04/text/original/epub/OEBPS/document_1/document_1.html#_Toc144218034> ;
    dcat:landingPage "https://www.legislation.gov.au/F2021L00313/2023-08-04/2023-08-04/text/original/epub/OEBPS/document_1/document_1.html#_Toc144218034"^^xsd:anyURI ;
    dcat:theme legcons:Item .

F2021L00313:19 a legcons:Item,
        owl:Class,
        dcat:Resource ;
    rdfs:label "Item - I19 2 2  Wild game meat and wild game meat products that are taken not to be prescribed goods"@en-AU ;
    dct:isPartOf F2021L00313:17 ;
    dct:isReferencedBy F2021L00313: ;
    rdfs:comment "2 2  Wild game meat and wild game meat products that are taken not to be prescribed goods - Abrievated Graph Key: I19"@en-AU ;
    skos:definition "2 2  Wild game meat and wild game meat products that are taken not to be prescribed goods"@en-AU ;
    skos:narrower F2021L00313:17 ;
    skos:prefLabel "Item I19"@en-AU ;
    dcat:accessURL <https://www.legislation.gov.au/F2021L00313/2023-08-04/2023-08-04/text/original/epub/OEBPS/document_1/document_1.html#_Toc144217864> ;
    dcat:landingPage "https://www.legislation.gov.au/F2021L00313/2023-08-04/2023-08-04/text/original/epub/OEBPS/document_1/document_1.html#_Toc144217864"^^xsd:anyURI ;
    dcat:theme legcons:Item .

F2021L00313:190 a legcons:Item,
        owl:Class,
        dcat:Resource ;
    rdfs:label "Item - I190 8 35  Persons who may manufacture supply or possess official marking devices"@en-AU ;
    dct:isPartOf F2021L00313:188 ;
    dct:isReferencedBy F2021L00313: ;
    rdfs:comment "8 35  Persons who may manufacture supply or possess official marking devices - Abrievated Graph Key: I190"@en-AU ;
    skos:definition "8 35  Persons who may manufacture supply or possess official marking devices"@en-AU ;
    skos:narrower F2021L00313:188 ;
    skos:prefLabel "Item I190"@en-AU ;
    dcat:accessURL <https://www.legislation.gov.au/F2021L00313/2023-08-04/2023-08-04/text/original/epub/OEBPS/document_1/document_1.html#_Toc144218035> ;
    dcat:landingPage "https://www.legislation.gov.au/F2021L00313/2023-08-04/2023-08-04/text/original/epub/OEBPS/document_1/document_1.html#_Toc144218035"^^xsd:anyURI ;
    dcat:theme legcons:Item .

F2021L00313:191 a legcons:Item,
        owl:Class,
        dcat:Resource ;
    rdfs:label "Item - I191 8 36  Security of official marking devices"@en-AU ;
    dct:isPartOf F2021L00313:188 ;
    dct:isReferencedBy F2021L00313: ;
    rdfs:comment "8 36  Security of official marking devices - Abrievated Graph Key: I191"@en-AU ;
    skos:definition "8 36  Security of official marking devices"@en-AU ;
    skos:narrower F2021L00313:188 ;
    skos:prefLabel "Item I191"@en-AU ;
    dcat:accessURL <https://www.legislation.gov.au/F2021L00313/2023-08-04/2023-08-04/text/original/epub/OEBPS/document_1/document_1.html#_Toc144218036> ;
    dcat:landingPage "https://www.legislation.gov.au/F2021L00313/2023-08-04/2023-08-04/text/original/epub/OEBPS/document_1/document_1.html#_Toc144218036"^^xsd:anyURI ;
    dcat:theme legcons:Item .

F2021L00313:192 a legcons:Item,
        owl:Class,
        dcat:Resource ;
    rdfs:label "Item - I192 8 37  Damaged etc official marking devices"@en-AU ;
    dct:isPartOf F2021L00313:188 ;
    dct:isReferencedBy F2021L00313: ;
    rdfs:comment "8 37  Damaged etc official marking devices - Abrievated Graph Key: I192"@en-AU ;
    skos:definition "8 37  Damaged etc official marking devices"@en-AU ;
    skos:narrower F2021L00313:188 ;
    skos:prefLabel "Item I192"@en-AU ;
    dcat:accessURL <https://www.legislation.gov.au/F2021L00313/2023-08-04/2023-08-04/text/original/epub/OEBPS/document_1/document_1.html#_Toc144218037> ;
    dcat:landingPage "https://www.legislation.gov.au/F2021L00313/2023-08-04/2023-08-04/text/original/epub/OEBPS/document_1/document_1.html#_Toc144218037"^^xsd:anyURI ;
    dcat:theme legcons:Item .

F2021L00313:193 a legcons:Item,
        owl:Class,
        dcat:Resource ;
    rdfs:label "Item - I193 8 38  Records of official marking devices manufactured or supplied"@en-AU ;
    dct:isPartOf F2021L00313:188 ;
    dct:isReferencedBy F2021L00313: ;
    rdfs:comment "8 38  Records of official marking devices manufactured or supplied - Abrievated Graph Key: I193"@en-AU ;
    skos:definition "8 38  Records of official marking devices manufactured or supplied"@en-AU ;
    skos:narrower F2021L00313:188 ;
    skos:prefLabel "Item I193"@en-AU ;
    dcat:accessURL <https://www.legislation.gov.au/F2021L00313/2023-08-04/2023-08-04/text/original/epub/OEBPS/document_1/document_1.html#_Toc144218038> ;
    dcat:landingPage "https://www.legislation.gov.au/F2021L00313/2023-08-04/2023-08-04/text/original/epub/OEBPS/document_1/document_1.html#_Toc144218038"^^xsd:anyURI ;
    dcat:theme legcons:Item .

F2021L00313:194 a legcons:Item,
        owl:Class,
        dcat:Resource ;
    rdfs:label "Item - I194 8 39  Records of official marking devices received used damaged destroyed or returned"@en-AU ;
    dct:isPartOf F2021L00313:188 ;
    dct:isReferencedBy F2021L00313: ;
    rdfs:comment "8 39  Records of official marking devices received used damaged destroyed or returned - Abrievated Graph Key: I194"@en-AU ;
    skos:definition "8 39  Records of official marking devices received used damaged destroyed or returned"@en-AU ;
    skos:narrower F2021L00313:188 ;
    skos:prefLabel "Item I194"@en-AU ;
    dcat:accessURL <https://www.legislation.gov.au/F2021L00313/2023-08-04/2023-08-04/text/original/epub/OEBPS/document_1/document_1.html#_Toc144218039> ;
    dcat:landingPage "https://www.legislation.gov.au/F2021L00313/2023-08-04/2023-08-04/text/original/epub/OEBPS/document_1/document_1.html#_Toc144218039"^^xsd:anyURI ;
    dcat:theme legcons:Item .

F2021L00313:198 a legcons:Item,
        owl:Class,
        dcat:Resource ;
    rdfs:label "Item - I198 9 1  References to audit in this Part"@en-AU ;
    dct:isPartOf F2021L00313:197 ;
    dct:isReferencedBy F2021L00313: ;
    rdfs:comment "9 1  References to audit in this Part - Abrievated Graph Key: I198"@en-AU ;
    skos:definition "9 1  References to audit in this Part"@en-AU ;
    skos:narrower F2021L00313:197 ;
    skos:prefLabel "Item I198"@en-AU ;
    dcat:accessURL <https://www.legislation.gov.au/F2021L00313/2023-08-04/2023-08-04/text/original/epub/OEBPS/document_1/document_1.html#_Toc144218043> ;
    dcat:landingPage "https://www.legislation.gov.au/F2021L00313/2023-08-04/2023-08-04/text/original/epub/OEBPS/document_1/document_1.html#_Toc144218043"^^xsd:anyURI ;
    dcat:theme legcons:Item .

F2021L00313:2 a legcons:Part,
        owl:Class,
        dcat:Resource ;
    rdfs:label "Part - P2 Part 1 Preliminary"@en-AU ;
    dct:isPartOf F2021L00313:1 ;
    dct:isReferencedBy F2021L00313: ;
    rdfs:comment "Part 1 Preliminary - Abrievated Graph Key: P2"@en-AU ;
    skos:definition "Part 1 Preliminary"@en-AU ;
    skos:narrower F2021L00313:1 ;
    skos:prefLabel "Part P2"@en-AU ;
    dcat:accessURL <https://www.legislation.gov.au/F2021L00313/2023-08-04/2023-08-04/text/original/epub/OEBPS/document_1/document_1.html#_Toc144217847> ;
    dcat:landingPage "https://www.legislation.gov.au/F2021L00313/2023-08-04/2023-08-04/text/original/epub/OEBPS/document_1/document_1.html#_Toc144217847"^^xsd:anyURI ;
    dcat:theme legcons:Part .

F2021L00313:200 a legcons:Item,
        owl:Class,
        dcat:Resource ;
    rdfs:label "Item - I200 9 2  Purpose of this Division"@en-AU ;
    dct:isPartOf F2021L00313:199 ;
    dct:isReferencedBy F2021L00313: ;
    rdfs:comment "9 2  Purpose of this Division - Abrievated Graph Key: I200"@en-AU ;
    skos:definition "9 2  Purpose of this Division"@en-AU ;
    skos:narrower F2021L00313:199 ;
    skos:prefLabel "Item I200"@en-AU ;
    dcat:accessURL <https://www.legislation.gov.au/F2021L00313/2023-08-04/2023-08-04/text/original/epub/OEBPS/document_1/document_1.html#_Toc144218045> ;
    dcat:landingPage "https://www.legislation.gov.au/F2021L00313/2023-08-04/2023-08-04/text/original/epub/OEBPS/document_1/document_1.html#_Toc144218045"^^xsd:anyURI ;
    dcat:theme legcons:Item .

F2021L00313:201 a legcons:Item,
        owl:Class,
        dcat:Resource ;
    rdfs:label "Item - I201 9 3  Manner in which audit must be conducted"@en-AU ;
    dct:isPartOf F2021L00313:199 ;
    dct:isReferencedBy F2021L00313: ;
    rdfs:comment "9 3  Manner in which audit must be conducted - Abrievated Graph Key: I201"@en-AU ;
    skos:definition "9 3  Manner in which audit must be conducted"@en-AU ;
    skos:narrower F2021L00313:199 ;
    skos:prefLabel "Item I201"@en-AU ;
    dcat:accessURL <https://www.legislation.gov.au/F2021L00313/2023-08-04/2023-08-04/text/original/epub/OEBPS/document_1/document_1.html#_Toc144218046> ;
    dcat:landingPage "https://www.legislation.gov.au/F2021L00313/2023-08-04/2023-08-04/text/original/epub/OEBPS/document_1/document_1.html#_Toc144218046"^^xsd:anyURI ;
    dcat:theme legcons:Item .

F2021L00313:202 a legcons:Item,
        owl:Class,
        dcat:Resource ;
    rdfs:label "Item - I202 9 4  Notice of non compliance with requirements"@en-AU ;
    dct:isPartOf F2021L00313:199 ;
    dct:isReferencedBy F2021L00313: ;
    rdfs:comment "9 4  Notice of non compliance with requirements - Abrievated Graph Key: I202"@en-AU ;
    skos:definition "9 4  Notice of non compliance with requirements"@en-AU ;
    skos:narrower F2021L00313:199 ;
    skos:prefLabel "Item I202"@en-AU ;
    dcat:accessURL <https://www.legislation.gov.au/F2021L00313/2023-08-04/2023-08-04/text/original/epub/OEBPS/document_1/document_1.html#_Toc144218047> ;
    dcat:landingPage "https://www.legislation.gov.au/F2021L00313/2023-08-04/2023-08-04/text/original/epub/OEBPS/document_1/document_1.html#_Toc144218047"^^xsd:anyURI ;
    dcat:theme legcons:Item .

F2021L00313:203 a legcons:Item,
        owl:Class,
        dcat:Resource ;
    rdfs:label "Item - I203 9 5  Audit reports"@en-AU ;
    dct:isPartOf F2021L00313:199 ;
    dct:isReferencedBy F2021L00313: ;
    rdfs:comment "9 5  Audit reports - Abrievated Graph Key: I203"@en-AU ;
    skos:definition "9 5  Audit reports"@en-AU ;
    skos:narrower F2021L00313:199 ;
    skos:prefLabel "Item I203"@en-AU ;
    dcat:accessURL <https://www.legislation.gov.au/F2021L00313/2023-08-04/2023-08-04/text/original/epub/OEBPS/document_1/document_1.html#_Toc144218048> ;
    dcat:landingPage "https://www.legislation.gov.au/F2021L00313/2023-08-04/2023-08-04/text/original/epub/OEBPS/document_1/document_1.html#_Toc144218048"^^xsd:anyURI ;
    dcat:theme legcons:Item .

F2021L00313:205 a legcons:Item,
        owl:Class,
        dcat:Resource ;
    rdfs:label "Item - I205 9 6  Purpose of this Division"@en-AU ;
    dct:isPartOf F2021L00313:204 ;
    dct:isReferencedBy F2021L00313: ;
    rdfs:comment "9 6  Purpose of this Division - Abrievated Graph Key: I205"@en-AU ;
    skos:definition "9 6  Purpose of this Division"@en-AU ;
    skos:narrower F2021L00313:204 ;
    skos:prefLabel "Item I205"@en-AU ;
    dcat:accessURL <https://www.legislation.gov.au/F2021L00313/2023-08-04/2023-08-04/text/original/epub/OEBPS/document_1/document_1.html#_Toc144218050> ;
    dcat:landingPage "https://www.legislation.gov.au/F2021L00313/2023-08-04/2023-08-04/text/original/epub/OEBPS/document_1/document_1.html#_Toc144218050"^^xsd:anyURI ;
    dcat:theme legcons:Item .

F2021L00313:206 a legcons:Item,
        owl:Class,
        dcat:Resource ;
    rdfs:label "Item - I206 9 7  Application for approval"@en-AU ;
    dct:isPartOf F2021L00313:204 ;
    dct:isReferencedBy F2021L00313: ;
    rdfs:comment "9 7  Application for approval - Abrievated Graph Key: I206"@en-AU ;
    skos:definition "9 7  Application for approval"@en-AU ;
    skos:narrower F2021L00313:204 ;
    skos:prefLabel "Item I206"@en-AU ;
    dcat:accessURL <https://www.legislation.gov.au/F2021L00313/2023-08-04/2023-08-04/text/original/epub/OEBPS/document_1/document_1.html#_Toc144218051> ;
    dcat:landingPage "https://www.legislation.gov.au/F2021L00313/2023-08-04/2023-08-04/text/original/epub/OEBPS/document_1/document_1.html#_Toc144218051"^^xsd:anyURI ;
    dcat:theme legcons:Item .

F2021L00313:207 a legcons:Item,
        owl:Class,
        dcat:Resource ;
    rdfs:label "Item - I207 9 8  Secretary must decide whether to approve applicant to conduct audits"@en-AU ;
    dct:isPartOf F2021L00313:204 ;
    dct:isReferencedBy F2021L00313: ;
    rdfs:comment "9 8  Secretary must decide whether to approve applicant to conduct audits - Abrievated Graph Key: I207"@en-AU ;
    skos:definition "9 8  Secretary must decide whether to approve applicant to conduct audits"@en-AU ;
    skos:narrower F2021L00313:204 ;
    skos:prefLabel "Item I207"@en-AU ;
    dcat:accessURL <https://www.legislation.gov.au/F2021L00313/2023-08-04/2023-08-04/text/original/epub/OEBPS/document_1/document_1.html#_Toc144218052> ;
    dcat:landingPage "https://www.legislation.gov.au/F2021L00313/2023-08-04/2023-08-04/text/original/epub/OEBPS/document_1/document_1.html#_Toc144218052"^^xsd:anyURI ;
    dcat:theme legcons:Item .

F2021L00313:208 a legcons:Item,
        owl:Class,
        dcat:Resource ;
    rdfs:label "Item - I208 9 9  Dealing with applications"@en-AU ;
    dct:isPartOf F2021L00313:204 ;
    dct:isReferencedBy F2021L00313: ;
    rdfs:comment "9 9  Dealing with applications - Abrievated Graph Key: I208"@en-AU ;
    skos:definition "9 9  Dealing with applications"@en-AU ;
    skos:narrower F2021L00313:204 ;
    skos:prefLabel "Item I208"@en-AU ;
    dcat:accessURL <https://www.legislation.gov.au/F2021L00313/2023-08-04/2023-08-04/text/original/epub/OEBPS/document_1/document_1.html#_Toc144218053> ;
    dcat:landingPage "https://www.legislation.gov.au/F2021L00313/2023-08-04/2023-08-04/text/original/epub/OEBPS/document_1/document_1.html#_Toc144218053"^^xsd:anyURI ;
    dcat:theme legcons:Item .

F2021L00313:209 a legcons:Item,
        owl:Class,
        dcat:Resource ;
    rdfs:label "Item - I209 9 10  Conditions of approval"@en-AU ;
    dct:isPartOf F2021L00313:204 ;
    dct:isReferencedBy F2021L00313: ;
    rdfs:comment "9 10  Conditions of approval - Abrievated Graph Key: I209"@en-AU ;
    skos:definition "9 10  Conditions of approval"@en-AU ;
    skos:narrower F2021L00313:204 ;
    skos:prefLabel "Item I209"@en-AU ;
    dcat:accessURL <https://www.legislation.gov.au/F2021L00313/2023-08-04/2023-08-04/text/original/epub/OEBPS/document_1/document_1.html#_Toc144218054> ;
    dcat:landingPage "https://www.legislation.gov.au/F2021L00313/2023-08-04/2023-08-04/text/original/epub/OEBPS/document_1/document_1.html#_Toc144218054"^^xsd:anyURI ;
    dcat:theme legcons:Item .

F2021L00313:21 a legcons:Item,
        owl:Class,
        dcat:Resource ;
    rdfs:label "Item - I21 2 3  Purpose and application of this Division"@en-AU ;
    dct:isPartOf F2021L00313:20 ;
    dct:isReferencedBy F2021L00313: ;
    rdfs:comment "2 3  Purpose and application of this Division - Abrievated Graph Key: I21"@en-AU ;
    skos:definition "2 3  Purpose and application of this Division"@en-AU ;
    skos:narrower F2021L00313:20 ;
    skos:prefLabel "Item I21"@en-AU ;
    dcat:accessURL <https://www.legislation.gov.au/F2021L00313/2023-08-04/2023-08-04/text/original/epub/OEBPS/document_1/document_1.html#_Toc144217866> ;
    dcat:landingPage "https://www.legislation.gov.au/F2021L00313/2023-08-04/2023-08-04/text/original/epub/OEBPS/document_1/document_1.html#_Toc144217866"^^xsd:anyURI ;
    dcat:theme legcons:Item .

F2021L00313:210 a legcons:Item,
        owl:Class,
        dcat:Resource ;
    rdfs:label "Item - I210 9 11  Notice of decision"@en-AU ;
    dct:isPartOf F2021L00313:204 ;
    dct:isReferencedBy F2021L00313: ;
    rdfs:comment "9 11  Notice of decision - Abrievated Graph Key: I210"@en-AU ;
    skos:definition "9 11  Notice of decision"@en-AU ;
    skos:narrower F2021L00313:204 ;
    skos:prefLabel "Item I210"@en-AU ;
    dcat:accessURL <https://www.legislation.gov.au/F2021L00313/2023-08-04/2023-08-04/text/original/epub/OEBPS/document_1/document_1.html#_Toc144218055> ;
    dcat:landingPage "https://www.legislation.gov.au/F2021L00313/2023-08-04/2023-08-04/text/original/epub/OEBPS/document_1/document_1.html#_Toc144218055"^^xsd:anyURI ;
    dcat:theme legcons:Item .

F2021L00313:211 a legcons:Item,
        owl:Class,
        dcat:Resource ;
    rdfs:label "Item - I211 9 12  Period of effect of approval"@en-AU ;
    dct:isPartOf F2021L00313:204 ;
    dct:isReferencedBy F2021L00313: ;
    rdfs:comment "9 12  Period of effect of approval - Abrievated Graph Key: I211"@en-AU ;
    skos:definition "9 12  Period of effect of approval"@en-AU ;
    skos:narrower F2021L00313:204 ;
    skos:prefLabel "Item I211"@en-AU ;
    dcat:accessURL <https://www.legislation.gov.au/F2021L00313/2023-08-04/2023-08-04/text/original/epub/OEBPS/document_1/document_1.html#_Toc144218056> ;
    dcat:landingPage "https://www.legislation.gov.au/F2021L00313/2023-08-04/2023-08-04/text/original/epub/OEBPS/document_1/document_1.html#_Toc144218056"^^xsd:anyURI ;
    dcat:theme legcons:Item .

F2021L00313:212 a legcons:Item,
        owl:Class,
        dcat:Resource ;
    rdfs:label "Item - I212 9 13  Imposing or varying conditions of approval"@en-AU ;
    dct:isPartOf F2021L00313:204 ;
    dct:isReferencedBy F2021L00313: ;
    rdfs:comment "9 13  Imposing or varying conditions of approval - Abrievated Graph Key: I212"@en-AU ;
    skos:definition "9 13  Imposing or varying conditions of approval"@en-AU ;
    skos:narrower F2021L00313:204 ;
    skos:prefLabel "Item I212"@en-AU ;
    dcat:accessURL <https://www.legislation.gov.au/F2021L00313/2023-08-04/2023-08-04/text/original/epub/OEBPS/document_1/document_1.html#_Toc144218057> ;
    dcat:landingPage "https://www.legislation.gov.au/F2021L00313/2023-08-04/2023-08-04/text/original/epub/OEBPS/document_1/document_1.html#_Toc144218057"^^xsd:anyURI ;
    dcat:theme legcons:Item .

F2021L00313:213 a legcons:Item,
        owl:Class,
        dcat:Resource ;
    rdfs:label "Item - I213 9 14  Revocation of approval"@en-AU ;
    dct:isPartOf F2021L00313:204 ;
    dct:isReferencedBy F2021L00313: ;
    rdfs:comment "9 14  Revocation of approval - Abrievated Graph Key: I213"@en-AU ;
    skos:definition "9 14  Revocation of approval"@en-AU ;
    skos:narrower F2021L00313:204 ;
    skos:prefLabel "Item I213"@en-AU ;
    dcat:accessURL <https://www.legislation.gov.au/F2021L00313/2023-08-04/2023-08-04/text/original/epub/OEBPS/document_1/document_1.html#_Toc144218058> ;
    dcat:landingPage "https://www.legislation.gov.au/F2021L00313/2023-08-04/2023-08-04/text/original/epub/OEBPS/document_1/document_1.html#_Toc144218058"^^xsd:anyURI ;
    dcat:theme legcons:Item .

F2021L00313:214 a legcons:Item,
        owl:Class,
        dcat:Resource ;
    rdfs:label "Item - I214 9 15  Register of approved auditors"@en-AU ;
    dct:isPartOf F2021L00313:204 ;
    dct:isReferencedBy F2021L00313: ;
    rdfs:comment "9 15  Register of approved auditors - Abrievated Graph Key: I214"@en-AU ;
    skos:definition "9 15  Register of approved auditors"@en-AU ;
    skos:narrower F2021L00313:204 ;
    skos:prefLabel "Item I214"@en-AU ;
    dcat:accessURL <https://www.legislation.gov.au/F2021L00313/2023-08-04/2023-08-04/text/original/epub/OEBPS/document_1/document_1.html#_Toc144218059> ;
    dcat:landingPage "https://www.legislation.gov.au/F2021L00313/2023-08-04/2023-08-04/text/original/epub/OEBPS/document_1/document_1.html#_Toc144218059"^^xsd:anyURI ;
    dcat:theme legcons:Item .

F2021L00313:215 a legcons:Item,
        owl:Class,
        dcat:Resource ;
    rdfs:label "Item - I215 9 16  Fit and proper person test"@en-AU ;
    dct:isPartOf F2021L00313:204 ;
    dct:isReferencedBy F2021L00313: ;
    rdfs:comment "9 16  Fit and proper person test - Abrievated Graph Key: I215"@en-AU ;
    skos:definition "9 16  Fit and proper person test"@en-AU ;
    skos:narrower F2021L00313:204 ;
    skos:prefLabel "Item I215"@en-AU ;
    dcat:accessURL <https://www.legislation.gov.au/F2021L00313/2023-08-04/2023-08-04/text/original/epub/OEBPS/document_1/document_1.html#_Toc144218060> ;
    dcat:landingPage "https://www.legislation.gov.au/F2021L00313/2023-08-04/2023-08-04/text/original/epub/OEBPS/document_1/document_1.html#_Toc144218060"^^xsd:anyURI ;
    dcat:theme legcons:Item .

F2021L00313:217 a legcons:Item,
        owl:Class,
        dcat:Resource ;
    rdfs:label "Item - I217 9 17  Circumstances in which assessment may be required or permitted"@en-AU ;
    dct:isPartOf F2021L00313:216 ;
    dct:isReferencedBy F2021L00313: ;
    rdfs:comment "9 17  Circumstances in which assessment may be required or permitted - Abrievated Graph Key: I217"@en-AU ;
    skos:definition "9 17  Circumstances in which assessment may be required or permitted"@en-AU ;
    skos:narrower F2021L00313:216 ;
    skos:prefLabel "Item I217"@en-AU ;
    dcat:accessURL <https://www.legislation.gov.au/F2021L00313/2023-08-04/2023-08-04/text/original/epub/OEBPS/document_1/document_1.html#_Toc144218062> ;
    dcat:landingPage "https://www.legislation.gov.au/F2021L00313/2023-08-04/2023-08-04/text/original/epub/OEBPS/document_1/document_1.html#_Toc144218062"^^xsd:anyURI ;
    dcat:theme legcons:Item .

F2021L00313:219 a legcons:Item,
        owl:Class,
        dcat:Resource ;
    rdfs:label "Item - I219 9 18  Decisions that may be made by operation of computer program"@en-AU ;
    dct:isPartOf F2021L00313:218 ;
    dct:isReferencedBy F2021L00313: ;
    rdfs:comment "9 18  Decisions that may be made by operation of computer program - Abrievated Graph Key: I219"@en-AU ;
    skos:definition "9 18  Decisions that may be made by operation of computer program"@en-AU ;
    skos:narrower F2021L00313:218 ;
    skos:prefLabel "Item I219"@en-AU ;
    dcat:accessURL <https://www.legislation.gov.au/F2021L00313/2023-08-04/2023-08-04/text/original/epub/OEBPS/document_1/document_1.html#_Toc144218064> ;
    dcat:landingPage "https://www.legislation.gov.au/F2021L00313/2023-08-04/2023-08-04/text/original/epub/OEBPS/document_1/document_1.html#_Toc144218064"^^xsd:anyURI ;
    dcat:theme legcons:Item .

F2021L00313:22 a legcons:Item,
        owl:Class,
        dcat:Resource ;
    rdfs:label "Item - I22 2 4  Export of prescribed wild game meat or wild game meat products is prohibited unless prescribed conditions are complied with"@en-AU ;
    dct:isPartOf F2021L00313:20 ;
    dct:isReferencedBy F2021L00313: ;
    rdfs:comment "2 4  Export of prescribed wild game meat or wild game meat products is prohibited unless prescribed conditions are complied with - Abrievated Graph Key: I22"@en-AU ;
    skos:definition "2 4  Export of prescribed wild game meat or wild game meat products is prohibited unless prescribed conditions are complied with"@en-AU ;
    skos:narrower F2021L00313:20 ;
    skos:prefLabel "Item I22"@en-AU ;
    dcat:accessURL <https://www.legislation.gov.au/F2021L00313/2023-08-04/2023-08-04/text/original/epub/OEBPS/document_1/document_1.html#_Toc144217867> ;
    dcat:landingPage "https://www.legislation.gov.au/F2021L00313/2023-08-04/2023-08-04/text/original/epub/OEBPS/document_1/document_1.html#_Toc144217867"^^xsd:anyURI ;
    dcat:theme legcons:Item .

F2021L00313:222 a legcons:Item,
        owl:Class,
        dcat:Resource ;
    rdfs:label "Item - I222 9 19  Requirement to be third party authorised officerfit and proper person etc"@en-AU ;
    dct:isPartOf F2021L00313:221 ;
    dct:isReferencedBy F2021L00313: ;
    rdfs:comment "9 19  Requirement to be third party authorised officerfit and proper person etc - Abrievated Graph Key: I222"@en-AU ;
    skos:definition "9 19  Requirement to be third party authorised officerfit and proper person etc"@en-AU ;
    skos:narrower F2021L00313:221 ;
    skos:prefLabel "Item I222"@en-AU ;
    dcat:accessURL <https://www.legislation.gov.au/F2021L00313/2023-08-04/2023-08-04/text/original/epub/OEBPS/document_1/document_1.html#_Toc144218067> ;
    dcat:landingPage "https://www.legislation.gov.au/F2021L00313/2023-08-04/2023-08-04/text/original/epub/OEBPS/document_1/document_1.html#_Toc144218067"^^xsd:anyURI ;
    dcat:theme legcons:Item .

F2021L00313:224 a legcons:Item,
        owl:Class,
        dcat:Resource ;
    rdfs:label "Item - I224 9 20  Purpose of this Division"@en-AU ;
    dct:isPartOf F2021L00313:223 ;
    dct:isReferencedBy F2021L00313: ;
    rdfs:comment "9 20  Purpose of this Division - Abrievated Graph Key: I224"@en-AU ;
    skos:definition "9 20  Purpose of this Division"@en-AU ;
    skos:narrower F2021L00313:223 ;
    skos:prefLabel "Item I224"@en-AU ;
    dcat:accessURL <https://www.legislation.gov.au/F2021L00313/2023-08-04/2023-08-04/text/original/epub/OEBPS/document_1/document_1.html#_Toc144218069> ;
    dcat:landingPage "https://www.legislation.gov.au/F2021L00313/2023-08-04/2023-08-04/text/original/epub/OEBPS/document_1/document_1.html#_Toc144218069"^^xsd:anyURI ;
    dcat:theme legcons:Item .

F2021L00313:225 a legcons:Item,
        owl:Class,
        dcat:Resource ;
    rdfs:label "Item - I225 9 21  Functions specified in Australian Wild Game Meat Standard and Australian Meat Standard"@en-AU ;
    dct:isPartOf F2021L00313:223 ;
    dct:isReferencedBy F2021L00313: ;
    rdfs:comment "9 21  Functions specified in Australian Wild Game Meat Standard and Australian Meat Standard - Abrievated Graph Key: I225"@en-AU ;
    skos:definition "9 21  Functions specified in Australian Wild Game Meat Standard and Australian Meat Standard"@en-AU ;
    skos:narrower F2021L00313:223 ;
    skos:prefLabel "Item I225"@en-AU ;
    dcat:accessURL <https://www.legislation.gov.au/F2021L00313/2023-08-04/2023-08-04/text/original/epub/OEBPS/document_1/document_1.html#_Toc144218070> ;
    dcat:landingPage "https://www.legislation.gov.au/F2021L00313/2023-08-04/2023-08-04/text/original/epub/OEBPS/document_1/document_1.html#_Toc144218070"^^xsd:anyURI ;
    dcat:theme legcons:Item .

F2021L00313:226 a legcons:Item,
        owl:Class,
        dcat:Resource ;
    rdfs:label "Item - I226 9 22  Inspections of carcases and carcase parts and applying post mortem dispositions"@en-AU ;
    dct:isPartOf F2021L00313:223 ;
    dct:isReferencedBy F2021L00313: ;
    rdfs:comment "9 22  Inspections of carcases and carcase parts and applying post mortem dispositions - Abrievated Graph Key: I226"@en-AU ;
    skos:definition "9 22  Inspections of carcases and carcase parts and applying post mortem dispositions"@en-AU ;
    skos:narrower F2021L00313:223 ;
    skos:prefLabel "Item I226"@en-AU ;
    dcat:accessURL <https://www.legislation.gov.au/F2021L00313/2023-08-04/2023-08-04/text/original/epub/OEBPS/document_1/document_1.html#_Toc144218071> ;
    dcat:landingPage "https://www.legislation.gov.au/F2021L00313/2023-08-04/2023-08-04/text/original/epub/OEBPS/document_1/document_1.html#_Toc144218071"^^xsd:anyURI ;
    dcat:theme legcons:Item .

F2021L00313:227 a legcons:Item,
        owl:Class,
        dcat:Resource ;
    rdfs:label "Item - I227 9 23  Inspections of wild game meat and wild game meat products and applying dispositions"@en-AU ;
    dct:isPartOf F2021L00313:223 ;
    dct:isReferencedBy F2021L00313: ;
    rdfs:comment "9 23  Inspections of wild game meat and wild game meat products and applying dispositions - Abrievated Graph Key: I227"@en-AU ;
    skos:definition "9 23  Inspections of wild game meat and wild game meat products and applying dispositions"@en-AU ;
    skos:narrower F2021L00313:223 ;
    skos:prefLabel "Item I227"@en-AU ;
    dcat:accessURL <https://www.legislation.gov.au/F2021L00313/2023-08-04/2023-08-04/text/original/epub/OEBPS/document_1/document_1.html#_Toc144218072> ;
    dcat:landingPage "https://www.legislation.gov.au/F2021L00313/2023-08-04/2023-08-04/text/original/epub/OEBPS/document_1/document_1.html#_Toc144218072"^^xsd:anyURI ;
    dcat:theme legcons:Item .

F2021L00313:228 a legcons:Item,
        owl:Class,
        dcat:Resource ;
    rdfs:label "Item - I228 9 24  Applying dispositions subject to conditions and variation"@en-AU ;
    dct:isPartOf F2021L00313:223 ;
    dct:isReferencedBy F2021L00313: ;
    rdfs:comment "9 24  Applying dispositions subject to conditions and variation - Abrievated Graph Key: I228"@en-AU ;
    skos:definition "9 24  Applying dispositions subject to conditions and variation"@en-AU ;
    skos:narrower F2021L00313:223 ;
    skos:prefLabel "Item I228"@en-AU ;
    dcat:accessURL <https://www.legislation.gov.au/F2021L00313/2023-08-04/2023-08-04/text/original/epub/OEBPS/document_1/document_1.html#_Toc144218073> ;
    dcat:landingPage "https://www.legislation.gov.au/F2021L00313/2023-08-04/2023-08-04/text/original/epub/OEBPS/document_1/document_1.html#_Toc144218073"^^xsd:anyURI ;
    dcat:theme legcons:Item .

F2021L00313:229 a legcons:Item,
        owl:Class,
        dcat:Resource ;
    rdfs:label "Item - I229 9 25  Stopping chain of operations temporarily or controlling rate of operations"@en-AU ;
    dct:isPartOf F2021L00313:223 ;
    dct:isReferencedBy F2021L00313: ;
    rdfs:comment "9 25  Stopping chain of operations temporarily or controlling rate of operations - Abrievated Graph Key: I229"@en-AU ;
    skos:definition "9 25  Stopping chain of operations temporarily or controlling rate of operations"@en-AU ;
    skos:narrower F2021L00313:223 ;
    skos:prefLabel "Item I229"@en-AU ;
    dcat:accessURL <https://www.legislation.gov.au/F2021L00313/2023-08-04/2023-08-04/text/original/epub/OEBPS/document_1/document_1.html#_Toc144218074> ;
    dcat:landingPage "https://www.legislation.gov.au/F2021L00313/2023-08-04/2023-08-04/text/original/epub/OEBPS/document_1/document_1.html#_Toc144218074"^^xsd:anyURI ;
    dcat:theme legcons:Item .

F2021L00313:230 a legcons:Item,
        owl:Class,
        dcat:Resource ;
    rdfs:label "Item - I230 9 26  Functions to be performed by veterinary officer or authorised officer acting under supervision of veterinary officer"@en-AU ;
    dct:isPartOf F2021L00313:223 ;
    dct:isReferencedBy F2021L00313: ;
    rdfs:comment "9 26  Functions to be performed by veterinary officer or authorised officer acting under supervision of veterinary officer - Abrievated Graph Key: I230"@en-AU ;
    skos:definition "9 26  Functions to be performed by veterinary officer or authorised officer acting under supervision of veterinary officer"@en-AU ;
    skos:narrower F2021L00313:223 ;
    skos:prefLabel "Item I230"@en-AU ;
    dcat:accessURL <https://www.legislation.gov.au/F2021L00313/2023-08-04/2023-08-04/text/original/epub/OEBPS/document_1/document_1.html#_Toc144218075> ;
    dcat:landingPage "https://www.legislation.gov.au/F2021L00313/2023-08-04/2023-08-04/text/original/epub/OEBPS/document_1/document_1.html#_Toc144218075"^^xsd:anyURI ;
    dcat:theme legcons:Item .

F2021L00313:231 a legcons:Item,
        owl:Class,
        dcat:Resource ;
    rdfs:label "Item - I231 9 27  Inspecting establishments and securing areas facilities equipment or other things"@en-AU ;
    dct:isPartOf F2021L00313:223 ;
    dct:isReferencedBy F2021L00313: ;
    rdfs:comment "9 27  Inspecting establishments and securing areas facilities equipment or other things - Abrievated Graph Key: I231"@en-AU ;
    skos:definition "9 27  Inspecting establishments and securing areas facilities equipment or other things"@en-AU ;
    skos:narrower F2021L00313:223 ;
    skos:prefLabel "Item I231"@en-AU ;
    dcat:accessURL <https://www.legislation.gov.au/F2021L00313/2023-08-04/2023-08-04/text/original/epub/OEBPS/document_1/document_1.html#_Toc144218076> ;
    dcat:landingPage "https://www.legislation.gov.au/F2021L00313/2023-08-04/2023-08-04/text/original/epub/OEBPS/document_1/document_1.html#_Toc144218076"^^xsd:anyURI ;
    dcat:theme legcons:Item .

F2021L00313:232 a legcons:Item,
        owl:Class,
        dcat:Resource ;
    rdfs:label "Item - I232 9 28  Securing and identifying establishment or conveyance etc"@en-AU ;
    dct:isPartOf F2021L00313:223 ;
    dct:isReferencedBy F2021L00313: ;
    rdfs:comment "9 28  Securing and identifying establishment or conveyance etc - Abrievated Graph Key: I232"@en-AU ;
    skos:definition "9 28  Securing and identifying establishment or conveyance etc"@en-AU ;
    skos:narrower F2021L00313:223 ;
    skos:prefLabel "Item I232"@en-AU ;
    dcat:accessURL <https://www.legislation.gov.au/F2021L00313/2023-08-04/2023-08-04/text/original/epub/OEBPS/document_1/document_1.html#_Toc144218077> ;
    dcat:landingPage "https://www.legislation.gov.au/F2021L00313/2023-08-04/2023-08-04/text/original/epub/OEBPS/document_1/document_1.html#_Toc144218077"^^xsd:anyURI ;
    dcat:theme legcons:Item .

F2021L00313:233 a legcons:Item,
        owl:Class,
        dcat:Resource ;
    rdfs:label "Item - I233 9 29  Interference with identified establishment or conveyance etc"@en-AU ;
    dct:isPartOf F2021L00313:223 ;
    dct:isReferencedBy F2021L00313: ;
    rdfs:comment "9 29  Interference with identified establishment or conveyance etc - Abrievated Graph Key: I233"@en-AU ;
    skos:definition "9 29  Interference with identified establishment or conveyance etc"@en-AU ;
    skos:narrower F2021L00313:223 ;
    skos:prefLabel "Item I233"@en-AU ;
    dcat:accessURL <https://www.legislation.gov.au/F2021L00313/2023-08-04/2023-08-04/text/original/epub/OEBPS/document_1/document_1.html#_Toc144218078> ;
    dcat:landingPage "https://www.legislation.gov.au/F2021L00313/2023-08-04/2023-08-04/text/original/epub/OEBPS/document_1/document_1.html#_Toc144218078"^^xsd:anyURI ;
    dcat:theme legcons:Item .

F2021L00313:234 a legcons:Item,
        owl:Class,
        dcat:Resource ;
    rdfs:label "Item - I234 9 30  Powers where integrity of prescribed wild game meat or wild game meat products may not be able to be ensured"@en-AU ;
    dct:isPartOf F2021L00313:223 ;
    dct:isReferencedBy F2021L00313: ;
    rdfs:comment "9 30  Powers where integrity of prescribed wild game meat or wild game meat products may not be able to be ensured - Abrievated Graph Key: I234"@en-AU ;
    skos:definition "9 30  Powers where integrity of prescribed wild game meat or wild game meat products may not be able to be ensured"@en-AU ;
    skos:narrower F2021L00313:223 ;
    skos:prefLabel "Item I234"@en-AU ;
    dcat:accessURL <https://www.legislation.gov.au/F2021L00313/2023-08-04/2023-08-04/text/original/epub/OEBPS/document_1/document_1.html#_Toc144218079> ;
    dcat:landingPage "https://www.legislation.gov.au/F2021L00313/2023-08-04/2023-08-04/text/original/epub/OEBPS/document_1/document_1.html#_Toc144218079"^^xsd:anyURI ;
    dcat:theme legcons:Item .

F2021L00313:235 a legcons:Item,
        owl:Class,
        dcat:Resource ;
    rdfs:label "Item - I235 9 31  Giving certificate of condemnation"@en-AU ;
    dct:isPartOf F2021L00313:223 ;
    dct:isReferencedBy F2021L00313: ;
    rdfs:comment "9 31  Giving certificate of condemnation - Abrievated Graph Key: I235"@en-AU ;
    skos:definition "9 31  Giving certificate of condemnation"@en-AU ;
    skos:narrower F2021L00313:223 ;
    skos:prefLabel "Item I235"@en-AU ;
    dcat:accessURL <https://www.legislation.gov.au/F2021L00313/2023-08-04/2023-08-04/text/original/epub/OEBPS/document_1/document_1.html#_Toc144218080> ;
    dcat:landingPage "https://www.legislation.gov.au/F2021L00313/2023-08-04/2023-08-04/text/original/epub/OEBPS/document_1/document_1.html#_Toc144218080"^^xsd:anyURI ;
    dcat:theme legcons:Item .

F2021L00313:237 a legcons:Item,
        owl:Class,
        dcat:Resource ;
    rdfs:label "Item - I237 9 32  Other grounds for giving direction"@en-AU ;
    dct:isPartOf F2021L00313:236 ;
    dct:isReferencedBy F2021L00313: ;
    rdfs:comment "9 32  Other grounds for giving direction - Abrievated Graph Key: I237"@en-AU ;
    skos:definition "9 32  Other grounds for giving direction"@en-AU ;
    skos:narrower F2021L00313:236 ;
    skos:prefLabel "Item I237"@en-AU ;
    dcat:accessURL <https://www.legislation.gov.au/F2021L00313/2023-08-04/2023-08-04/text/original/epub/OEBPS/document_1/document_1.html#_Toc144218082> ;
    dcat:landingPage "https://www.legislation.gov.au/F2021L00313/2023-08-04/2023-08-04/text/original/epub/OEBPS/document_1/document_1.html#_Toc144218082"^^xsd:anyURI ;
    dcat:theme legcons:Item .

F2021L00313:239 a legcons:Item,
        owl:Class,
        dcat:Resource ;
    rdfs:label "Item - I239 9 33  Circumstances in which identity card need not be carried"@en-AU ;
    dct:isPartOf F2021L00313:238 ;
    dct:isReferencedBy F2021L00313: ;
    rdfs:comment "9 33  Circumstances in which identity card need not be carried - Abrievated Graph Key: I239"@en-AU ;
    skos:definition "9 33  Circumstances in which identity card need not be carried"@en-AU ;
    skos:narrower F2021L00313:238 ;
    skos:prefLabel "Item I239"@en-AU ;
    dcat:accessURL <https://www.legislation.gov.au/F2021L00313/2023-08-04/2023-08-04/text/original/epub/OEBPS/document_1/document_1.html#_Toc144218084> ;
    dcat:landingPage "https://www.legislation.gov.au/F2021L00313/2023-08-04/2023-08-04/text/original/epub/OEBPS/document_1/document_1.html#_Toc144218084"^^xsd:anyURI ;
    dcat:theme legcons:Item .

F2021L00313:24 a legcons:Item,
        owl:Class,
        dcat:Resource ;
    rdfs:label "Item - I24 2 5  Application of this Part"@en-AU ;
    dct:isPartOf F2021L00313:23 ;
    dct:isReferencedBy F2021L00313: ;
    rdfs:comment "2 5  Application of this Part - Abrievated Graph Key: I24"@en-AU ;
    skos:definition "2 5  Application of this Part"@en-AU ;
    skos:narrower F2021L00313:23 ;
    skos:prefLabel "Item I24"@en-AU ;
    dcat:accessURL <https://www.legislation.gov.au/F2021L00313/2023-08-04/2023-08-04/text/original/epub/OEBPS/document_1/document_1.html#_Toc144217869> ;
    dcat:landingPage "https://www.legislation.gov.au/F2021L00313/2023-08-04/2023-08-04/text/original/epub/OEBPS/document_1/document_1.html#_Toc144217869"^^xsd:anyURI ;
    dcat:theme legcons:Item .

F2021L00313:241 a legcons:Item,
        owl:Class,
        dcat:Resource ;
    rdfs:label "Item - I241 10 1  Samples taken in exercising monitoring or investigation powers"@en-AU ;
    dct:isPartOf F2021L00313:240 ;
    dct:isReferencedBy F2021L00313: ;
    rdfs:comment "10 1  Samples taken in exercising monitoring or investigation powers - Abrievated Graph Key: I241"@en-AU ;
    skos:definition "10 1  Samples taken in exercising monitoring or investigation powers"@en-AU ;
    skos:narrower F2021L00313:240 ;
    skos:prefLabel "Item I241"@en-AU ;
    dcat:accessURL <https://www.legislation.gov.au/F2021L00313/2023-08-04/2023-08-04/text/original/epub/OEBPS/document_1/document_1.html#_Toc144218086> ;
    dcat:landingPage "https://www.legislation.gov.au/F2021L00313/2023-08-04/2023-08-04/text/original/epub/OEBPS/document_1/document_1.html#_Toc144218086"^^xsd:anyURI ;
    dcat:theme legcons:Item .

F2021L00313:242 a legcons:Item,
        owl:Class,
        dcat:Resource ;
    rdfs:label "Item - I242 10 2  Dealing with things seized in exercising investigation powers"@en-AU ;
    dct:isPartOf F2021L00313:240 ;
    dct:isReferencedBy F2021L00313: ;
    rdfs:comment "10 2  Dealing with things seized in exercising investigation powers - Abrievated Graph Key: I242"@en-AU ;
    skos:definition "10 2  Dealing with things seized in exercising investigation powers"@en-AU ;
    skos:narrower F2021L00313:240 ;
    skos:prefLabel "Item I242"@en-AU ;
    dcat:accessURL <https://www.legislation.gov.au/F2021L00313/2023-08-04/2023-08-04/text/original/epub/OEBPS/document_1/document_1.html#_Toc144218087> ;
    dcat:landingPage "https://www.legislation.gov.au/F2021L00313/2023-08-04/2023-08-04/text/original/epub/OEBPS/document_1/document_1.html#_Toc144218087"^^xsd:anyURI ;
    dcat:theme legcons:Item .

F2021L00313:245 a legcons:Item,
        owl:Class,
        dcat:Resource ;
    rdfs:label "Item - I245 11 1  Reviewable decisions"@en-AU ;
    dct:isPartOf F2021L00313:244 ;
    dct:isReferencedBy F2021L00313: ;
    rdfs:comment "11 1  Reviewable decisions - Abrievated Graph Key: I245"@en-AU ;
    skos:definition "11 1  Reviewable decisions"@en-AU ;
    skos:narrower F2021L00313:244 ;
    skos:prefLabel "Item I245"@en-AU ;
    dcat:accessURL <https://www.legislation.gov.au/F2021L00313/2023-08-04/2023-08-04/text/original/epub/OEBPS/document_1/document_1.html#_Toc144218090> ;
    dcat:landingPage "https://www.legislation.gov.au/F2021L00313/2023-08-04/2023-08-04/text/original/epub/OEBPS/document_1/document_1.html#_Toc144218090"^^xsd:anyURI ;
    dcat:theme legcons:Item .

F2021L00313:247 a legcons:Item,
        owl:Class,
        dcat:Resource ;
    rdfs:label "Item - I247 11 2  Purpose of this Part"@en-AU ;
    dct:isPartOf F2021L00313:246 ;
    dct:isReferencedBy F2021L00313: ;
    rdfs:comment "11 2  Purpose of this Part - Abrievated Graph Key: I247"@en-AU ;
    skos:definition "11 2  Purpose of this Part"@en-AU ;
    skos:narrower F2021L00313:246 ;
    skos:prefLabel "Item I247"@en-AU ;
    dcat:accessURL <https://www.legislation.gov.au/F2021L00313/2023-08-04/2023-08-04/text/original/epub/OEBPS/document_1/document_1.html#_Toc144218092> ;
    dcat:landingPage "https://www.legislation.gov.au/F2021L00313/2023-08-04/2023-08-04/text/original/epub/OEBPS/document_1/document_1.html#_Toc144218092"^^xsd:anyURI ;
    dcat:theme legcons:Item .

F2021L00313:248 a legcons:Item,
        owl:Class,
        dcat:Resource ;
    rdfs:label "Item - I248 11 3  General requirements for records"@en-AU ;
    dct:isPartOf F2021L00313:246 ;
    dct:isReferencedBy F2021L00313: ;
    rdfs:comment "11 3  General requirements for records - Abrievated Graph Key: I248"@en-AU ;
    skos:definition "11 3  General requirements for records"@en-AU ;
    skos:narrower F2021L00313:246 ;
    skos:prefLabel "Item I248"@en-AU ;
    dcat:accessURL <https://www.legislation.gov.au/F2021L00313/2023-08-04/2023-08-04/text/original/epub/OEBPS/document_1/document_1.html#_Toc144218093> ;
    dcat:landingPage "https://www.legislation.gov.au/F2021L00313/2023-08-04/2023-08-04/text/original/epub/OEBPS/document_1/document_1.html#_Toc144218093"^^xsd:anyURI ;
    dcat:theme legcons:Item .

F2021L00313:249 a legcons:Item,
        owl:Class,
        dcat:Resource ;
    rdfs:label "Item - I249 11 4  Government certificates"@en-AU ;
    dct:isPartOf F2021L00313:246 ;
    dct:isReferencedBy F2021L00313: ;
    rdfs:comment "11 4  Government certificates - Abrievated Graph Key: I249"@en-AU ;
    skos:definition "11 4  Government certificates"@en-AU ;
    skos:narrower F2021L00313:246 ;
    skos:prefLabel "Item I249"@en-AU ;
    dcat:accessURL <https://www.legislation.gov.au/F2021L00313/2023-08-04/2023-08-04/text/original/epub/OEBPS/document_1/document_1.html#_Toc144218094> ;
    dcat:landingPage "https://www.legislation.gov.au/F2021L00313/2023-08-04/2023-08-04/text/original/epub/OEBPS/document_1/document_1.html#_Toc144218094"^^xsd:anyURI ;
    dcat:theme legcons:Item .

F2021L00313:25 a legcons:Item,
        owl:Class,
        dcat:Resource ;
    rdfs:label "Item - I25 2 6  Period for making application for exemption"@en-AU ;
    dct:isPartOf F2021L00313:23 ;
    dct:isReferencedBy F2021L00313: ;
    rdfs:comment "2 6  Period for making application for exemption - Abrievated Graph Key: I25"@en-AU ;
    skos:definition "2 6  Period for making application for exemption"@en-AU ;
    skos:narrower F2021L00313:23 ;
    skos:prefLabel "Item I25"@en-AU ;
    dcat:accessURL <https://www.legislation.gov.au/F2021L00313/2023-08-04/2023-08-04/text/original/epub/OEBPS/document_1/document_1.html#_Toc144217870> ;
    dcat:landingPage "https://www.legislation.gov.au/F2021L00313/2023-08-04/2023-08-04/text/original/epub/OEBPS/document_1/document_1.html#_Toc144217870"^^xsd:anyURI ;
    dcat:theme legcons:Item .

F2021L00313:250 a legcons:Item,
        owl:Class,
        dcat:Resource ;
    rdfs:label "Item - I250 11 5  Export permits"@en-AU ;
    dct:isPartOf F2021L00313:246 ;
    dct:isReferencedBy F2021L00313: ;
    rdfs:comment "11 5  Export permits - Abrievated Graph Key: I250"@en-AU ;
    skos:definition "11 5  Export permits"@en-AU ;
    skos:narrower F2021L00313:246 ;
    skos:prefLabel "Item I250"@en-AU ;
    dcat:accessURL <https://www.legislation.gov.au/F2021L00313/2023-08-04/2023-08-04/text/original/epub/OEBPS/document_1/document_1.html#_Toc144218095> ;
    dcat:landingPage "https://www.legislation.gov.au/F2021L00313/2023-08-04/2023-08-04/text/original/epub/OEBPS/document_1/document_1.html#_Toc144218095"^^xsd:anyURI ;
    dcat:theme legcons:Item .

F2021L00313:251 a legcons:Item,
        owl:Class,
        dcat:Resource ;
    rdfs:label "Item - I251 11 6  Records to be retained by exporter"@en-AU ;
    dct:isPartOf F2021L00313:246 ;
    dct:isReferencedBy F2021L00313: ;
    rdfs:comment "11 6  Records to be retained by exporter - Abrievated Graph Key: I251"@en-AU ;
    skos:definition "11 6  Records to be retained by exporter"@en-AU ;
    skos:narrower F2021L00313:246 ;
    skos:prefLabel "Item I251"@en-AU ;
    dcat:accessURL <https://www.legislation.gov.au/F2021L00313/2023-08-04/2023-08-04/text/original/epub/OEBPS/document_1/document_1.html#_Toc144218096> ;
    dcat:landingPage "https://www.legislation.gov.au/F2021L00313/2023-08-04/2023-08-04/text/original/epub/OEBPS/document_1/document_1.html#_Toc144218096"^^xsd:anyURI ;
    dcat:theme legcons:Item .

F2021L00313:252 a legcons:Item,
        owl:Class,
        dcat:Resource ;
    rdfs:label "Item - I252 11 7  Records to be retained by occupier of registered establishment"@en-AU ;
    dct:isPartOf F2021L00313:246 ;
    dct:isReferencedBy F2021L00313: ;
    rdfs:comment "11 7  Records to be retained by occupier of registered establishment - Abrievated Graph Key: I252"@en-AU ;
    skos:definition "11 7  Records to be retained by occupier of registered establishment"@en-AU ;
    skos:narrower F2021L00313:246 ;
    skos:prefLabel "Item I252"@en-AU ;
    dcat:accessURL <https://www.legislation.gov.au/F2021L00313/2023-08-04/2023-08-04/text/original/epub/OEBPS/document_1/document_1.html#_Toc144218097> ;
    dcat:landingPage "https://www.legislation.gov.au/F2021L00313/2023-08-04/2023-08-04/text/original/epub/OEBPS/document_1/document_1.html#_Toc144218097"^^xsd:anyURI ;
    dcat:theme legcons:Item .

F2021L00313:253 a legcons:Item,
        owl:Class,
        dcat:Resource ;
    rdfs:label "Item - I253 11 8  Records to be retained by holder of approved arrangement"@en-AU ;
    dct:isPartOf F2021L00313:246 ;
    dct:isReferencedBy F2021L00313: ;
    rdfs:comment "11 8  Records to be retained by holder of approved arrangement - Abrievated Graph Key: I253"@en-AU ;
    skos:definition "11 8  Records to be retained by holder of approved arrangement"@en-AU ;
    skos:narrower F2021L00313:246 ;
    skos:prefLabel "Item I253"@en-AU ;
    dcat:accessURL <https://www.legislation.gov.au/F2021L00313/2023-08-04/2023-08-04/text/original/epub/OEBPS/document_1/document_1.html#_Toc144218098> ;
    dcat:landingPage "https://www.legislation.gov.au/F2021L00313/2023-08-04/2023-08-04/text/original/epub/OEBPS/document_1/document_1.html#_Toc144218098"^^xsd:anyURI ;
    dcat:theme legcons:Item .

F2021L00313:254 a legcons:Item,
        owl:Class,
        dcat:Resource ;
    rdfs:label "Item - I254 11 9  Records relating to official marks"@en-AU ;
    dct:isPartOf F2021L00313:246 ;
    dct:isReferencedBy F2021L00313: ;
    rdfs:comment "11 9  Records relating to official marks - Abrievated Graph Key: I254"@en-AU ;
    skos:definition "11 9  Records relating to official marks"@en-AU ;
    skos:narrower F2021L00313:246 ;
    skos:prefLabel "Item I254"@en-AU ;
    dcat:accessURL <https://www.legislation.gov.au/F2021L00313/2023-08-04/2023-08-04/text/original/epub/OEBPS/document_1/document_1.html#_Toc144218099> ;
    dcat:landingPage "https://www.legislation.gov.au/F2021L00313/2023-08-04/2023-08-04/text/original/epub/OEBPS/document_1/document_1.html#_Toc144218099"^^xsd:anyURI ;
    dcat:theme legcons:Item .

F2021L00313:255 a legcons:Item,
        owl:Class,
        dcat:Resource ;
    rdfs:label "Item - I255 11 10  Records relating to official marking devices"@en-AU ;
    dct:isPartOf F2021L00313:246 ;
    dct:isReferencedBy F2021L00313: ;
    rdfs:comment "11 10  Records relating to official marking devices - Abrievated Graph Key: I255"@en-AU ;
    skos:definition "11 10  Records relating to official marking devices"@en-AU ;
    skos:narrower F2021L00313:246 ;
    skos:prefLabel "Item I255"@en-AU ;
    dcat:accessURL <https://www.legislation.gov.au/F2021L00313/2023-08-04/2023-08-04/text/original/epub/OEBPS/document_1/document_1.html#_Toc144218100> ;
    dcat:landingPage "https://www.legislation.gov.au/F2021L00313/2023-08-04/2023-08-04/text/original/epub/OEBPS/document_1/document_1.html#_Toc144218100"^^xsd:anyURI ;
    dcat:theme legcons:Item .

F2021L00313:256 a legcons:Item,
        owl:Class,
        dcat:Resource ;
    rdfs:label "Item - I256 11 11  Records must not be altered or defaced during retention period"@en-AU ;
    dct:isPartOf F2021L00313:246 ;
    dct:isReferencedBy F2021L00313: ;
    rdfs:comment "11 11  Records must not be altered or defaced during retention period - Abrievated Graph Key: I256"@en-AU ;
    skos:definition "11 11  Records must not be altered or defaced during retention period"@en-AU ;
    skos:narrower F2021L00313:246 ;
    skos:prefLabel "Item I256"@en-AU ;
    dcat:accessURL <https://www.legislation.gov.au/F2021L00313/2023-08-04/2023-08-04/text/original/epub/OEBPS/document_1/document_1.html#_Toc144218101> ;
    dcat:landingPage "https://www.legislation.gov.au/F2021L00313/2023-08-04/2023-08-04/text/original/epub/OEBPS/document_1/document_1.html#_Toc144218101"^^xsd:anyURI ;
    dcat:theme legcons:Item .

F2021L00313:258 a legcons:Item,
        owl:Class,
        dcat:Resource ;
    rdfs:label "Item - I258 11 12  Storage of samples"@en-AU ;
    dct:isPartOf F2021L00313:257 ;
    dct:isReferencedBy F2021L00313: ;
    rdfs:comment "11 12  Storage of samples - Abrievated Graph Key: I258"@en-AU ;
    skos:definition "11 12  Storage of samples"@en-AU ;
    skos:narrower F2021L00313:257 ;
    skos:prefLabel "Item I258"@en-AU ;
    dcat:accessURL <https://www.legislation.gov.au/F2021L00313/2023-08-04/2023-08-04/text/original/epub/OEBPS/document_1/document_1.html#_Toc144218103> ;
    dcat:landingPage "https://www.legislation.gov.au/F2021L00313/2023-08-04/2023-08-04/text/original/epub/OEBPS/document_1/document_1.html#_Toc144218103"^^xsd:anyURI ;
    dcat:theme legcons:Item .

F2021L00313:26 a legcons:Item,
        owl:Class,
        dcat:Resource ;
    rdfs:label "Item - I26 2 7  Conditions of exemptionmatters to which Secretary must have regard"@en-AU ;
    dct:isPartOf F2021L00313:23 ;
    dct:isReferencedBy F2021L00313: ;
    rdfs:comment "2 7  Conditions of exemptionmatters to which Secretary must have regard - Abrievated Graph Key: I26"@en-AU ;
    skos:definition "2 7  Conditions of exemptionmatters to which Secretary must have regard"@en-AU ;
    skos:narrower F2021L00313:23 ;
    skos:prefLabel "Item I26"@en-AU ;
    dcat:accessURL <https://www.legislation.gov.au/F2021L00313/2023-08-04/2023-08-04/text/original/epub/OEBPS/document_1/document_1.html#_Toc144217871> ;
    dcat:landingPage "https://www.legislation.gov.au/F2021L00313/2023-08-04/2023-08-04/text/original/epub/OEBPS/document_1/document_1.html#_Toc144217871"^^xsd:anyURI ;
    dcat:theme legcons:Item .

F2021L00313:260 a legcons:Item,
        owl:Class,
        dcat:Resource ;
    rdfs:label "Item - I260 11 13  Division of compensation between owners"@en-AU ;
    dct:isPartOf F2021L00313:259 ;
    dct:isReferencedBy F2021L00313: ;
    rdfs:comment "11 13  Division of compensation between owners - Abrievated Graph Key: I260"@en-AU ;
    skos:definition "11 13  Division of compensation between owners"@en-AU ;
    skos:narrower F2021L00313:259 ;
    skos:prefLabel "Item I260"@en-AU ;
    dcat:accessURL <https://www.legislation.gov.au/F2021L00313/2023-08-04/2023-08-04/text/original/epub/OEBPS/document_1/document_1.html#_Toc144218105> ;
    dcat:landingPage "https://www.legislation.gov.au/F2021L00313/2023-08-04/2023-08-04/text/original/epub/OEBPS/document_1/document_1.html#_Toc144218105"^^xsd:anyURI ;
    dcat:theme legcons:Item .

F2021L00313:261 a legcons:Item,
        owl:Class,
        dcat:Resource ;
    rdfs:label "Item - I261 11 14  Amount of compensation"@en-AU ;
    dct:isPartOf F2021L00313:259 ;
    dct:isReferencedBy F2021L00313: ;
    rdfs:comment "11 14  Amount of compensation - Abrievated Graph Key: I261"@en-AU ;
    skos:definition "11 14  Amount of compensation"@en-AU ;
    skos:narrower F2021L00313:259 ;
    skos:prefLabel "Item I261"@en-AU ;
    dcat:accessURL <https://www.legislation.gov.au/F2021L00313/2023-08-04/2023-08-04/text/original/epub/OEBPS/document_1/document_1.html#_Toc144218106> ;
    dcat:landingPage "https://www.legislation.gov.au/F2021L00313/2023-08-04/2023-08-04/text/original/epub/OEBPS/document_1/document_1.html#_Toc144218106"^^xsd:anyURI ;
    dcat:theme legcons:Item .

F2021L00313:263 a legcons:Item,
        owl:Class,
        dcat:Resource ;
    rdfs:label "Item - I263 11 15  Circumstances in which relevant Commonwealth liability of a person is taken to have been paid"@en-AU ;
    dct:isPartOf F2021L00313:262 ;
    dct:isReferencedBy F2021L00313: ;
    rdfs:comment "11 15  Circumstances in which relevant Commonwealth liability of a person is taken to have been paid - Abrievated Graph Key: I263"@en-AU ;
    skos:definition "11 15  Circumstances in which relevant Commonwealth liability of a person is taken to have been paid"@en-AU ;
    skos:narrower F2021L00313:262 ;
    skos:prefLabel "Item I263"@en-AU ;
    dcat:accessURL <https://www.legislation.gov.au/F2021L00313/2023-08-04/2023-08-04/text/original/epub/OEBPS/document_1/document_1.html#_Toc144218108> ;
    dcat:landingPage "https://www.legislation.gov.au/F2021L00313/2023-08-04/2023-08-04/text/original/epub/OEBPS/document_1/document_1.html#_Toc144218108"^^xsd:anyURI ;
    dcat:theme legcons:Item .

F2021L00313:266 a legcons:Item,
        owl:Class,
        dcat:Resource ;
    rdfs:label "Item - I266 12 1  Definitions"@en-AU ;
    dct:isPartOf F2021L00313:265 ;
    dct:isReferencedBy F2021L00313: ;
    rdfs:comment "12 1  Definitions - Abrievated Graph Key: I266"@en-AU ;
    skos:definition "12 1  Definitions"@en-AU ;
    skos:narrower F2021L00313:265 ;
    skos:prefLabel "Item I266"@en-AU ;
    dcat:accessURL <https://www.legislation.gov.au/F2021L00313/2023-08-04/2023-08-04/text/original/epub/OEBPS/document_1/document_1.html#_Toc144218111> ;
    dcat:landingPage "https://www.legislation.gov.au/F2021L00313/2023-08-04/2023-08-04/text/original/epub/OEBPS/document_1/document_1.html#_Toc144218111"^^xsd:anyURI ;
    dcat:theme legcons:Item .

F2021L00313:268 a legcons:Item,
        owl:Class,
        dcat:Resource ;
    rdfs:label "Item - I268 12 2  Allocations of inspection services in effect immediately before commencement time"@en-AU ;
    dct:isPartOf F2021L00313:267 ;
    dct:isReferencedBy F2021L00313: ;
    rdfs:comment "12 2  Allocations of inspection services in effect immediately before commencement time - Abrievated Graph Key: I268"@en-AU ;
    skos:definition "12 2  Allocations of inspection services in effect immediately before commencement time"@en-AU ;
    skos:narrower F2021L00313:267 ;
    skos:prefLabel "Item I268"@en-AU ;
    dcat:accessURL <https://www.legislation.gov.au/F2021L00313/2023-08-04/2023-08-04/text/original/epub/OEBPS/document_1/document_1.html#_Toc144218113> ;
    dcat:landingPage "https://www.legislation.gov.au/F2021L00313/2023-08-04/2023-08-04/text/original/epub/OEBPS/document_1/document_1.html#_Toc144218113"^^xsd:anyURI ;
    dcat:theme legcons:Item .

F2021L00313:269 a legcons:Item,
        owl:Class,
        dcat:Resource ;
    rdfs:label "Item - I269 12 3  Application for inspection services not decided or notice of decision not given before commencement time"@en-AU ;
    dct:isPartOf F2021L00313:267 ;
    dct:isReferencedBy F2021L00313: ;
    rdfs:comment "12 3  Application for inspection services not decided or notice of decision not given before commencement time - Abrievated Graph Key: I269"@en-AU ;
    skos:definition "12 3  Application for inspection services not decided or notice of decision not given before commencement time"@en-AU ;
    skos:narrower F2021L00313:267 ;
    skos:prefLabel "Item I269"@en-AU ;
    dcat:accessURL <https://www.legislation.gov.au/F2021L00313/2023-08-04/2023-08-04/text/original/epub/OEBPS/document_1/document_1.html#_Toc144218114> ;
    dcat:landingPage "https://www.legislation.gov.au/F2021L00313/2023-08-04/2023-08-04/text/original/epub/OEBPS/document_1/document_1.html#_Toc144218114"^^xsd:anyURI ;
    dcat:theme legcons:Item .

F2021L00313:27 a legcons:Item,
        owl:Class,
        dcat:Resource ;
    rdfs:label "Item - I27 2 8  Period of effect of exemption"@en-AU ;
    dct:isPartOf F2021L00313:23 ;
    dct:isReferencedBy F2021L00313: ;
    rdfs:comment "2 8  Period of effect of exemption - Abrievated Graph Key: I27"@en-AU ;
    skos:definition "2 8  Period of effect of exemption"@en-AU ;
    skos:narrower F2021L00313:23 ;
    skos:prefLabel "Item I27"@en-AU ;
    dcat:accessURL <https://www.legislation.gov.au/F2021L00313/2023-08-04/2023-08-04/text/original/epub/OEBPS/document_1/document_1.html#_Toc144217872> ;
    dcat:landingPage "https://www.legislation.gov.au/F2021L00313/2023-08-04/2023-08-04/text/original/epub/OEBPS/document_1/document_1.html#_Toc144217872"^^xsd:anyURI ;
    dcat:theme legcons:Item .

F2021L00313:270 a legcons:Item,
        owl:Class,
        dcat:Resource ;
    rdfs:label "Item - I270 12 4  Notice of preliminary determination of allocation given before commencement time"@en-AU ;
    dct:isPartOf F2021L00313:267 ;
    dct:isReferencedBy F2021L00313: ;
    rdfs:comment "12 4  Notice of preliminary determination of allocation given before commencement time - Abrievated Graph Key: I270"@en-AU ;
    skos:definition "12 4  Notice of preliminary determination of allocation given before commencement time"@en-AU ;
    skos:narrower F2021L00313:267 ;
    skos:prefLabel "Item I270"@en-AU ;
    dcat:accessURL <https://www.legislation.gov.au/F2021L00313/2023-08-04/2023-08-04/text/original/epub/OEBPS/document_1/document_1.html#_Toc144218115> ;
    dcat:landingPage "https://www.legislation.gov.au/F2021L00313/2023-08-04/2023-08-04/text/original/epub/OEBPS/document_1/document_1.html#_Toc144218115"^^xsd:anyURI ;
    dcat:theme legcons:Item .

F2021L00313:271 a legcons:Item,
        owl:Class,
        dcat:Resource ;
    rdfs:label "Item - I271 12 5  Preliminary determination of allocation agreed before commencement time"@en-AU ;
    dct:isPartOf F2021L00313:267 ;
    dct:isReferencedBy F2021L00313: ;
    rdfs:comment "12 5  Preliminary determination of allocation agreed before commencement time - Abrievated Graph Key: I271"@en-AU ;
    skos:definition "12 5  Preliminary determination of allocation agreed before commencement time"@en-AU ;
    skos:narrower F2021L00313:267 ;
    skos:prefLabel "Item I271"@en-AU ;
    dcat:accessURL <https://www.legislation.gov.au/F2021L00313/2023-08-04/2023-08-04/text/original/epub/OEBPS/document_1/document_1.html#_Toc144218116> ;
    dcat:landingPage "https://www.legislation.gov.au/F2021L00313/2023-08-04/2023-08-04/text/original/epub/OEBPS/document_1/document_1.html#_Toc144218116"^^xsd:anyURI ;
    dcat:theme legcons:Item .

F2021L00313:272 a legcons:Item,
        owl:Class,
        dcat:Resource ;
    rdfs:label "Item - I272 12 6  Revised determination made but notice not given before commencement time"@en-AU ;
    dct:isPartOf F2021L00313:267 ;
    dct:isReferencedBy F2021L00313: ;
    rdfs:comment "12 6  Revised determination made but notice not given before commencement time - Abrievated Graph Key: I272"@en-AU ;
    skos:definition "12 6  Revised determination made but notice not given before commencement time"@en-AU ;
    skos:narrower F2021L00313:267 ;
    skos:prefLabel "Item I272"@en-AU ;
    dcat:accessURL <https://www.legislation.gov.au/F2021L00313/2023-08-04/2023-08-04/text/original/epub/OEBPS/document_1/document_1.html#_Toc144218117> ;
    dcat:landingPage "https://www.legislation.gov.au/F2021L00313/2023-08-04/2023-08-04/text/original/epub/OEBPS/document_1/document_1.html#_Toc144218117"^^xsd:anyURI ;
    dcat:theme legcons:Item .

F2021L00313:273 a legcons:Item,
        owl:Class,
        dcat:Resource ;
    rdfs:label "Item - I273 12 7  Notice of revised determination of inspection services given before commencement time"@en-AU ;
    dct:isPartOf F2021L00313:267 ;
    dct:isReferencedBy F2021L00313: ;
    rdfs:comment "12 7  Notice of revised determination of inspection services given before commencement time - Abrievated Graph Key: I273"@en-AU ;
    skos:definition "12 7  Notice of revised determination of inspection services given before commencement time"@en-AU ;
    skos:narrower F2021L00313:267 ;
    skos:prefLabel "Item I273"@en-AU ;
    dcat:accessURL <https://www.legislation.gov.au/F2021L00313/2023-08-04/2023-08-04/text/original/epub/OEBPS/document_1/document_1.html#_Toc144218118> ;
    dcat:landingPage "https://www.legislation.gov.au/F2021L00313/2023-08-04/2023-08-04/text/original/epub/OEBPS/document_1/document_1.html#_Toc144218118"^^xsd:anyURI ;
    dcat:theme legcons:Item .

F2021L00313:274 a legcons:Item,
        owl:Class,
        dcat:Resource ;
    rdfs:label "Item - I274 12 8  Revised determination of allocation agreed before commencement time"@en-AU ;
    dct:isPartOf F2021L00313:267 ;
    dct:isReferencedBy F2021L00313: ;
    rdfs:comment "12 8  Revised determination of allocation agreed before commencement time - Abrievated Graph Key: I274"@en-AU ;
    skos:definition "12 8  Revised determination of allocation agreed before commencement time"@en-AU ;
    skos:narrower F2021L00313:267 ;
    skos:prefLabel "Item I274"@en-AU ;
    dcat:accessURL <https://www.legislation.gov.au/F2021L00313/2023-08-04/2023-08-04/text/original/epub/OEBPS/document_1/document_1.html#_Toc144218119> ;
    dcat:landingPage "https://www.legislation.gov.au/F2021L00313/2023-08-04/2023-08-04/text/original/epub/OEBPS/document_1/document_1.html#_Toc144218119"^^xsd:anyURI ;
    dcat:theme legcons:Item .

F2021L00313:275 a legcons:Item,
        owl:Class,
        dcat:Resource ;
    rdfs:label "Item - I275 12 9  Application for review committee made but committee not established before commencement time"@en-AU ;
    dct:isPartOf F2021L00313:267 ;
    dct:isReferencedBy F2021L00313: ;
    rdfs:comment "12 9  Application for review committee made but committee not established before commencement time - Abrievated Graph Key: I275"@en-AU ;
    skos:definition "12 9  Application for review committee made but committee not established before commencement time"@en-AU ;
    skos:narrower F2021L00313:267 ;
    skos:prefLabel "Item I275"@en-AU ;
    dcat:accessURL <https://www.legislation.gov.au/F2021L00313/2023-08-04/2023-08-04/text/original/epub/OEBPS/document_1/document_1.html#_Toc144218120> ;
    dcat:landingPage "https://www.legislation.gov.au/F2021L00313/2023-08-04/2023-08-04/text/original/epub/OEBPS/document_1/document_1.html#_Toc144218120"^^xsd:anyURI ;
    dcat:theme legcons:Item .

F2021L00313:276 a legcons:Item,
        owl:Class,
        dcat:Resource ;
    rdfs:label "Item - I276 12 10  Committee review in progress before commencement time"@en-AU ;
    dct:isPartOf F2021L00313:267 ;
    dct:isReferencedBy F2021L00313: ;
    rdfs:comment "12 10  Committee review in progress before commencement time - Abrievated Graph Key: I276"@en-AU ;
    skos:definition "12 10  Committee review in progress before commencement time"@en-AU ;
    skos:narrower F2021L00313:267 ;
    skos:prefLabel "Item I276"@en-AU ;
    dcat:accessURL <https://www.legislation.gov.au/F2021L00313/2023-08-04/2023-08-04/text/original/epub/OEBPS/document_1/document_1.html#_Toc144218121> ;
    dcat:landingPage "https://www.legislation.gov.au/F2021L00313/2023-08-04/2023-08-04/text/original/epub/OEBPS/document_1/document_1.html#_Toc144218121"^^xsd:anyURI ;
    dcat:theme legcons:Item .

F2021L00313:277 a legcons:Item,
        owl:Class,
        dcat:Resource ;
    rdfs:label "Item - I277 12 11  Determination reconsidered but notice not given before commencement time"@en-AU ;
    dct:isPartOf F2021L00313:267 ;
    dct:isReferencedBy F2021L00313: ;
    rdfs:comment "12 11  Determination reconsidered but notice not given before commencement time - Abrievated Graph Key: I277"@en-AU ;
    skos:definition "12 11  Determination reconsidered but notice not given before commencement time"@en-AU ;
    skos:narrower F2021L00313:267 ;
    skos:prefLabel "Item I277"@en-AU ;
    dcat:accessURL <https://www.legislation.gov.au/F2021L00313/2023-08-04/2023-08-04/text/original/epub/OEBPS/document_1/document_1.html#_Toc144218122> ;
    dcat:landingPage "https://www.legislation.gov.au/F2021L00313/2023-08-04/2023-08-04/text/original/epub/OEBPS/document_1/document_1.html#_Toc144218122"^^xsd:anyURI ;
    dcat:theme legcons:Item .

F2021L00313:278 a legcons:Item,
        owl:Class,
        dcat:Resource ;
    rdfs:label "Item - I278 12 12  Application to alter inspection services not decided before commencement time"@en-AU ;
    dct:isPartOf F2021L00313:267 ;
    dct:isReferencedBy F2021L00313: ;
    rdfs:comment "12 12  Application to alter inspection services not decided before commencement time - Abrievated Graph Key: I278"@en-AU ;
    skos:definition "12 12  Application to alter inspection services not decided before commencement time"@en-AU ;
    skos:narrower F2021L00313:267 ;
    skos:prefLabel "Item I278"@en-AU ;
    dcat:accessURL <https://www.legislation.gov.au/F2021L00313/2023-08-04/2023-08-04/text/original/epub/OEBPS/document_1/document_1.html#_Toc144218123> ;
    dcat:landingPage "https://www.legislation.gov.au/F2021L00313/2023-08-04/2023-08-04/text/original/epub/OEBPS/document_1/document_1.html#_Toc144218123"^^xsd:anyURI ;
    dcat:theme legcons:Item .

F2021L00313:279 a legcons:Item,
        owl:Class,
        dcat:Resource ;
    rdfs:label "Item - I279 12 13  Application for additional inspection services not decided before commencement time"@en-AU ;
    dct:isPartOf F2021L00313:267 ;
    dct:isReferencedBy F2021L00313: ;
    rdfs:comment "12 13  Application for additional inspection services not decided before commencement time - Abrievated Graph Key: I279"@en-AU ;
    skos:definition "12 13  Application for additional inspection services not decided before commencement time"@en-AU ;
    skos:narrower F2021L00313:267 ;
    skos:prefLabel "Item I279"@en-AU ;
    dcat:accessURL <https://www.legislation.gov.au/F2021L00313/2023-08-04/2023-08-04/text/original/epub/OEBPS/document_1/document_1.html#_Toc144218124> ;
    dcat:landingPage "https://www.legislation.gov.au/F2021L00313/2023-08-04/2023-08-04/text/original/epub/OEBPS/document_1/document_1.html#_Toc144218124"^^xsd:anyURI ;
    dcat:theme legcons:Item .

F2021L00313:28 a legcons:Item,
        owl:Class,
        dcat:Resource ;
    rdfs:label "Item - I28 2 9  Variation of conditions of exemptionmatters to which Secretary must have regard"@en-AU ;
    dct:isPartOf F2021L00313:23 ;
    dct:isReferencedBy F2021L00313: ;
    rdfs:comment "2 9  Variation of conditions of exemptionmatters to which Secretary must have regard - Abrievated Graph Key: I28"@en-AU ;
    skos:definition "2 9  Variation of conditions of exemptionmatters to which Secretary must have regard"@en-AU ;
    skos:narrower F2021L00313:23 ;
    skos:prefLabel "Item I28"@en-AU ;
    dcat:accessURL <https://www.legislation.gov.au/F2021L00313/2023-08-04/2023-08-04/text/original/epub/OEBPS/document_1/document_1.html#_Toc144217873> ;
    dcat:landingPage "https://www.legislation.gov.au/F2021L00313/2023-08-04/2023-08-04/text/original/epub/OEBPS/document_1/document_1.html#_Toc144217873"^^xsd:anyURI ;
    dcat:theme legcons:Item .

F2021L00313:280 a legcons:Item,
        owl:Class,
        dcat:Resource ;
    rdfs:label "Item - I280 12 14  Notice of termination of additional inspection services given before commencement time"@en-AU ;
    dct:isPartOf F2021L00313:267 ;
    dct:isReferencedBy F2021L00313: ;
    rdfs:comment "12 14  Notice of termination of additional inspection services given before commencement time - Abrievated Graph Key: I280"@en-AU ;
    skos:definition "12 14  Notice of termination of additional inspection services given before commencement time"@en-AU ;
    skos:narrower F2021L00313:267 ;
    skos:prefLabel "Item I280"@en-AU ;
    dcat:accessURL <https://www.legislation.gov.au/F2021L00313/2023-08-04/2023-08-04/text/original/epub/OEBPS/document_1/document_1.html#_Toc144218125> ;
    dcat:landingPage "https://www.legislation.gov.au/F2021L00313/2023-08-04/2023-08-04/text/original/epub/OEBPS/document_1/document_1.html#_Toc144218125"^^xsd:anyURI ;
    dcat:theme legcons:Item .

F2021L00313:281 a legcons:Item,
        owl:Class,
        dcat:Resource ;
    rdfs:label "Item - I281 12 15  Notice of shutdown given before commencement time"@en-AU ;
    dct:isPartOf F2021L00313:267 ;
    dct:isReferencedBy F2021L00313: ;
    rdfs:comment "12 15  Notice of shutdown given before commencement time - Abrievated Graph Key: I281"@en-AU ;
    skos:definition "12 15  Notice of shutdown given before commencement time"@en-AU ;
    skos:narrower F2021L00313:267 ;
    skos:prefLabel "Item I281"@en-AU ;
    dcat:accessURL <https://www.legislation.gov.au/F2021L00313/2023-08-04/2023-08-04/text/original/epub/OEBPS/document_1/document_1.html#_Toc144218126> ;
    dcat:landingPage "https://www.legislation.gov.au/F2021L00313/2023-08-04/2023-08-04/text/original/epub/OEBPS/document_1/document_1.html#_Toc144218126"^^xsd:anyURI ;
    dcat:theme legcons:Item .

F2021L00313:282 a legcons:Item,
        owl:Class,
        dcat:Resource ;
    rdfs:label "Item - I282 12 16  Variation of allocation for change of circumstance not advised before commencement time"@en-AU ;
    dct:isPartOf F2021L00313:267 ;
    dct:isReferencedBy F2021L00313: ;
    rdfs:comment "12 16  Variation of allocation for change of circumstance not advised before commencement time - Abrievated Graph Key: I282"@en-AU ;
    skos:definition "12 16  Variation of allocation for change of circumstance not advised before commencement time"@en-AU ;
    skos:narrower F2021L00313:267 ;
    skos:prefLabel "Item I282"@en-AU ;
    dcat:accessURL <https://www.legislation.gov.au/F2021L00313/2023-08-04/2023-08-04/text/original/epub/OEBPS/document_1/document_1.html#_Toc144218127> ;
    dcat:landingPage "https://www.legislation.gov.au/F2021L00313/2023-08-04/2023-08-04/text/original/epub/OEBPS/document_1/document_1.html#_Toc144218127"^^xsd:anyURI ;
    dcat:theme legcons:Item .

F2021L00313:283 a legcons:Item,
        owl:Class,
        dcat:Resource ;
    rdfs:label "Item - I283 12 17  Disputed allocation not decided before commencement time"@en-AU ;
    dct:isPartOf F2021L00313:267 ;
    dct:isReferencedBy F2021L00313: ;
    rdfs:comment "12 17  Disputed allocation not decided before commencement time - Abrievated Graph Key: I283"@en-AU ;
    skos:definition "12 17  Disputed allocation not decided before commencement time"@en-AU ;
    skos:narrower F2021L00313:267 ;
    skos:prefLabel "Item I283"@en-AU ;
    dcat:accessURL <https://www.legislation.gov.au/F2021L00313/2023-08-04/2023-08-04/text/original/epub/OEBPS/document_1/document_1.html#_Toc144218128> ;
    dcat:landingPage "https://www.legislation.gov.au/F2021L00313/2023-08-04/2023-08-04/text/original/epub/OEBPS/document_1/document_1.html#_Toc144218128"^^xsd:anyURI ;
    dcat:theme legcons:Item .

F2021L00313:284 a legcons:Item,
        owl:Class,
        dcat:Resource ;
    rdfs:label "Item - I284 12 18  Notice of reconsideration of disputed allocation not given before commencement time"@en-AU ;
    dct:isPartOf F2021L00313:267 ;
    dct:isReferencedBy F2021L00313: ;
    rdfs:comment "12 18  Notice of reconsideration of disputed allocation not given before commencement time - Abrievated Graph Key: I284"@en-AU ;
    skos:definition "12 18  Notice of reconsideration of disputed allocation not given before commencement time"@en-AU ;
    skos:narrower F2021L00313:267 ;
    skos:prefLabel "Item I284"@en-AU ;
    dcat:accessURL <https://www.legislation.gov.au/F2021L00313/2023-08-04/2023-08-04/text/original/epub/OEBPS/document_1/document_1.html#_Toc144218129> ;
    dcat:landingPage "https://www.legislation.gov.au/F2021L00313/2023-08-04/2023-08-04/text/original/epub/OEBPS/document_1/document_1.html#_Toc144218129"^^xsd:anyURI ;
    dcat:theme legcons:Item .

F2021L00313:286 a legcons:Item,
        owl:Class,
        dcat:Resource ;
    rdfs:label "Item - I286 12 19  Information and declarations given before commencement time"@en-AU ;
    dct:isPartOf F2021L00313:285 ;
    dct:isReferencedBy F2021L00313: ;
    rdfs:comment "12 19  Information and declarations given before commencement time - Abrievated Graph Key: I286"@en-AU ;
    skos:definition "12 19  Information and declarations given before commencement time"@en-AU ;
    skos:narrower F2021L00313:285 ;
    skos:prefLabel "Item I286"@en-AU ;
    dcat:accessURL <https://www.legislation.gov.au/F2021L00313/2023-08-04/2023-08-04/text/original/epub/OEBPS/document_1/document_1.html#_Toc144218131> ;
    dcat:landingPage "https://www.legislation.gov.au/F2021L00313/2023-08-04/2023-08-04/text/original/epub/OEBPS/document_1/document_1.html#_Toc144218131"^^xsd:anyURI ;
    dcat:theme legcons:Item .

F2021L00313:289 a legcons:Item,
        owl:Class,
        dcat:Resource ;
    rdfs:label "Item - I289 12 20  Request for translation not complied with before commencement time"@en-AU ;
    dct:isPartOf F2021L00313:288 ;
    dct:isReferencedBy F2021L00313: ;
    rdfs:comment "12 20  Request for translation not complied with before commencement time - Abrievated Graph Key: I289"@en-AU ;
    skos:definition "12 20  Request for translation not complied with before commencement time"@en-AU ;
    skos:narrower F2021L00313:288 ;
    skos:prefLabel "Item I289"@en-AU ;
    dcat:accessURL <https://www.legislation.gov.au/F2021L00313/2023-08-04/2023-08-04/text/original/epub/OEBPS/document_1/document_1.html#_Toc144218134> ;
    dcat:landingPage "https://www.legislation.gov.au/F2021L00313/2023-08-04/2023-08-04/text/original/epub/OEBPS/document_1/document_1.html#_Toc144218134"^^xsd:anyURI ;
    dcat:theme legcons:Item .

F2021L00313:29 a legcons:Item,
        owl:Class,
        dcat:Resource ;
    rdfs:label "Item - I29 2 10  Revocation of exemptionmatters to which Secretary must have regard"@en-AU ;
    dct:isPartOf F2021L00313:23 ;
    dct:isReferencedBy F2021L00313: ;
    rdfs:comment "2 10  Revocation of exemptionmatters to which Secretary must have regard - Abrievated Graph Key: I29"@en-AU ;
    skos:definition "2 10  Revocation of exemptionmatters to which Secretary must have regard"@en-AU ;
    skos:narrower F2021L00313:23 ;
    skos:prefLabel "Item I29"@en-AU ;
    dcat:accessURL <https://www.legislation.gov.au/F2021L00313/2023-08-04/2023-08-04/text/original/epub/OEBPS/document_1/document_1.html#_Toc144217874> ;
    dcat:landingPage "https://www.legislation.gov.au/F2021L00313/2023-08-04/2023-08-04/text/original/epub/OEBPS/document_1/document_1.html#_Toc144217874"^^xsd:anyURI ;
    dcat:theme legcons:Item .

F2021L00313:291 a legcons:Item,
        owl:Class,
        dcat:Resource ;
    rdfs:label "Item - I291 12 21  Person approved before commencement time to manufacture an official mark"@en-AU ;
    dct:isPartOf F2021L00313:290 ;
    dct:isReferencedBy F2021L00313: ;
    rdfs:comment "12 21  Person approved before commencement time to manufacture an official mark - Abrievated Graph Key: I291"@en-AU ;
    skos:definition "12 21  Person approved before commencement time to manufacture an official mark"@en-AU ;
    skos:narrower F2021L00313:290 ;
    skos:prefLabel "Item I291"@en-AU ;
    dcat:accessURL <https://www.legislation.gov.au/F2021L00313/2023-08-04/2023-08-04/text/original/epub/OEBPS/document_1/document_1.html#_Toc144218136> ;
    dcat:landingPage "https://www.legislation.gov.au/F2021L00313/2023-08-04/2023-08-04/text/original/epub/OEBPS/document_1/document_1.html#_Toc144218136"^^xsd:anyURI ;
    dcat:theme legcons:Item .

F2021L00313:292 a legcons:Item,
        owl:Class,
        dcat:Resource ;
    rdfs:label "Item - I292 12 22  Person approved before commencement time to apply an official mark"@en-AU ;
    dct:isPartOf F2021L00313:290 ;
    dct:isReferencedBy F2021L00313: ;
    rdfs:comment "12 22  Person approved before commencement time to apply an official mark - Abrievated Graph Key: I292"@en-AU ;
    skos:definition "12 22  Person approved before commencement time to apply an official mark"@en-AU ;
    skos:narrower F2021L00313:290 ;
    skos:prefLabel "Item I292"@en-AU ;
    dcat:accessURL <https://www.legislation.gov.au/F2021L00313/2023-08-04/2023-08-04/text/original/epub/OEBPS/document_1/document_1.html#_Toc144218137> ;
    dcat:landingPage "https://www.legislation.gov.au/F2021L00313/2023-08-04/2023-08-04/text/original/epub/OEBPS/document_1/document_1.html#_Toc144218137"^^xsd:anyURI ;
    dcat:theme legcons:Item .

F2021L00313:294 a legcons:Item,
        owl:Class,
        dcat:Resource ;
    rdfs:label "Item - I294 12 23  Person approved before commencement time to manufacture an official marking device"@en-AU ;
    dct:isPartOf F2021L00313:293 ;
    dct:isReferencedBy F2021L00313: ;
    rdfs:comment "12 23  Person approved before commencement time to manufacture an official marking device - Abrievated Graph Key: I294"@en-AU ;
    skos:definition "12 23  Person approved before commencement time to manufacture an official marking device"@en-AU ;
    skos:narrower F2021L00313:293 ;
    skos:prefLabel "Item I294"@en-AU ;
    dcat:accessURL <https://www.legislation.gov.au/F2021L00313/2023-08-04/2023-08-04/text/original/epub/OEBPS/document_1/document_1.html#_Toc144218139> ;
    dcat:landingPage "https://www.legislation.gov.au/F2021L00313/2023-08-04/2023-08-04/text/original/epub/OEBPS/document_1/document_1.html#_Toc144218139"^^xsd:anyURI ;
    dcat:theme legcons:Item .

F2021L00313:295 a legcons:Item,
        owl:Class,
        dcat:Resource ;
    rdfs:label "Item - I295 12 24  Person approved before commencement time to possess an official marking device"@en-AU ;
    dct:isPartOf F2021L00313:293 ;
    dct:isReferencedBy F2021L00313: ;
    rdfs:comment "12 24  Person approved before commencement time to possess an official marking device - Abrievated Graph Key: I295"@en-AU ;
    skos:definition "12 24  Person approved before commencement time to possess an official marking device"@en-AU ;
    skos:narrower F2021L00313:293 ;
    skos:prefLabel "Item I295"@en-AU ;
    dcat:accessURL <https://www.legislation.gov.au/F2021L00313/2023-08-04/2023-08-04/text/original/epub/OEBPS/document_1/document_1.html#_Toc144218140> ;
    dcat:landingPage "https://www.legislation.gov.au/F2021L00313/2023-08-04/2023-08-04/text/original/epub/OEBPS/document_1/document_1.html#_Toc144218140"^^xsd:anyURI ;
    dcat:theme legcons:Item .

F2021L00313:298 a legcons:Item,
        owl:Class,
        dcat:Resource ;
    rdfs:label "Item - I298 12 25  Application for approval as auditor not decided or notice of decision not given before commencement time"@en-AU ;
    dct:isPartOf F2021L00313:297 ;
    dct:isReferencedBy F2021L00313: ;
    rdfs:comment "12 25  Application for approval as auditor not decided or notice of decision not given before commencement time - Abrievated Graph Key: I298"@en-AU ;
    skos:definition "12 25  Application for approval as auditor not decided or notice of decision not given before commencement time"@en-AU ;
    skos:narrower F2021L00313:297 ;
    skos:prefLabel "Item I298"@en-AU ;
    dcat:accessURL <https://www.legislation.gov.au/F2021L00313/2023-08-04/2023-08-04/text/original/epub/OEBPS/document_1/document_1.html#_Toc144218143> ;
    dcat:landingPage "https://www.legislation.gov.au/F2021L00313/2023-08-04/2023-08-04/text/original/epub/OEBPS/document_1/document_1.html#_Toc144218143"^^xsd:anyURI ;
    dcat:theme legcons:Item .

F2021L00313:299 a legcons:Item,
        owl:Class,
        dcat:Resource ;
    rdfs:label "Item - I299 12 26  Request for further information not complied with before commencement time"@en-AU ;
    dct:isPartOf F2021L00313:297 ;
    dct:isReferencedBy F2021L00313: ;
    rdfs:comment "12 26  Request for further information not complied with before commencement time - Abrievated Graph Key: I299"@en-AU ;
    skos:definition "12 26  Request for further information not complied with before commencement time"@en-AU ;
    skos:narrower F2021L00313:297 ;
    skos:prefLabel "Item I299"@en-AU ;
    dcat:accessURL <https://www.legislation.gov.au/F2021L00313/2023-08-04/2023-08-04/text/original/epub/OEBPS/document_1/document_1.html#_Toc144218144> ;
    dcat:landingPage "https://www.legislation.gov.au/F2021L00313/2023-08-04/2023-08-04/text/original/epub/OEBPS/document_1/document_1.html#_Toc144218144"^^xsd:anyURI ;
    dcat:theme legcons:Item .

F2021L00313:3 a legcons:Item,
        owl:Class,
        dcat:Resource ;
    rdfs:label "Item - I3 1 1  Name"@en-AU ;
    dct:isPartOf F2021L00313:1 ;
    dct:isReferencedBy F2021L00313: ;
    rdfs:comment "1 1  Name - Abrievated Graph Key: I3"@en-AU ;
    skos:definition "1 1  Name"@en-AU ;
    skos:narrower F2021L00313:1 ;
    skos:prefLabel "Item I3"@en-AU ;
    dcat:accessURL <https://www.legislation.gov.au/F2021L00313/2023-08-04/2023-08-04/text/original/epub/OEBPS/document_1/document_1.html#_Toc144217848> ;
    dcat:landingPage "https://www.legislation.gov.au/F2021L00313/2023-08-04/2023-08-04/text/original/epub/OEBPS/document_1/document_1.html#_Toc144217848"^^xsd:anyURI ;
    dcat:theme legcons:Item .

F2021L00313:300 a legcons:Item,
        owl:Class,
        dcat:Resource ;
    rdfs:label "Item - I300 12 27  Decision to revoke approval as auditor decided but notice not given before commencement time"@en-AU ;
    dct:isPartOf F2021L00313:297 ;
    dct:isReferencedBy F2021L00313: ;
    rdfs:comment "12 27  Decision to revoke approval as auditor decided but notice not given before commencement time - Abrievated Graph Key: I300"@en-AU ;
    skos:definition "12 27  Decision to revoke approval as auditor decided but notice not given before commencement time"@en-AU ;
    skos:narrower F2021L00313:297 ;
    skos:prefLabel "Item I300"@en-AU ;
    dcat:accessURL <https://www.legislation.gov.au/F2021L00313/2023-08-04/2023-08-04/text/original/epub/OEBPS/document_1/document_1.html#_Toc144218145> ;
    dcat:landingPage "https://www.legislation.gov.au/F2021L00313/2023-08-04/2023-08-04/text/original/epub/OEBPS/document_1/document_1.html#_Toc144218145"^^xsd:anyURI ;
    dcat:theme legcons:Item .

F2021L00313:302 a legcons:Item,
        owl:Class,
        dcat:Resource ;
    rdfs:label "Item - I302 12 28  Disposition applied but not complied with before commencement time"@en-AU ;
    dct:isPartOf F2021L00313:301 ;
    dct:isReferencedBy F2021L00313: ;
    rdfs:comment "12 28  Disposition applied but not complied with before commencement time - Abrievated Graph Key: I302"@en-AU ;
    skos:definition "12 28  Disposition applied but not complied with before commencement time"@en-AU ;
    skos:narrower F2021L00313:301 ;
    skos:prefLabel "Item I302"@en-AU ;
    dcat:accessURL <https://www.legislation.gov.au/F2021L00313/2023-08-04/2023-08-04/text/original/epub/OEBPS/document_1/document_1.html#_Toc144218147> ;
    dcat:landingPage "https://www.legislation.gov.au/F2021L00313/2023-08-04/2023-08-04/text/original/epub/OEBPS/document_1/document_1.html#_Toc144218147"^^xsd:anyURI ;
    dcat:theme legcons:Item .

F2021L00313:303 a legcons:Item,
        owl:Class,
        dcat:Resource ;
    rdfs:label "Item - I303 12 29  Certificate of condemnation requested but not given before commencement time"@en-AU ;
    dct:isPartOf F2021L00313:301 ;
    dct:isReferencedBy F2021L00313: ;
    rdfs:comment "12 29  Certificate of condemnation requested but not given before commencement time - Abrievated Graph Key: I303"@en-AU ;
    skos:definition "12 29  Certificate of condemnation requested but not given before commencement time"@en-AU ;
    skos:narrower F2021L00313:301 ;
    skos:prefLabel "Item I303"@en-AU ;
    dcat:accessURL <https://www.legislation.gov.au/F2021L00313/2023-08-04/2023-08-04/text/original/epub/OEBPS/document_1/document_1.html#_Toc144218148> ;
    dcat:landingPage "https://www.legislation.gov.au/F2021L00313/2023-08-04/2023-08-04/text/original/epub/OEBPS/document_1/document_1.html#_Toc144218148"^^xsd:anyURI ;
    dcat:theme legcons:Item .

F2021L00313:305 a legcons:Item,
        owl:Class,
        dcat:Resource ;
    rdfs:label "Item - I305 Endnote 1 About the endnotes"@en-AU ;
    dct:isPartOf F2021L00313:304 ;
    dct:isReferencedBy F2021L00313: ;
    rdfs:comment "Endnote 1 About the endnotes - Abrievated Graph Key: I305"@en-AU ;
    skos:definition "Endnote 1 About the endnotes"@en-AU ;
    skos:narrower F2021L00313:304 ;
    skos:prefLabel "Item I305"@en-AU ;
    dcat:accessURL <https://www.legislation.gov.au/F2021L00313/2023-08-04/2023-08-04/text/original/epub/OEBPS/document_1/document_1.html#_Toc144218150> ;
    dcat:landingPage "https://www.legislation.gov.au/F2021L00313/2023-08-04/2023-08-04/text/original/epub/OEBPS/document_1/document_1.html#_Toc144218150"^^xsd:anyURI ;
    dcat:theme legcons:Item .

F2021L00313:306 a legcons:Item,
        owl:Class,
        dcat:Resource ;
    rdfs:label "Item - I306 Endnote 2 Abbreviation key"@en-AU ;
    dct:isPartOf F2021L00313:304 ;
    dct:isReferencedBy F2021L00313: ;
    rdfs:comment "Endnote 2 Abbreviation key - Abrievated Graph Key: I306"@en-AU ;
    skos:definition "Endnote 2 Abbreviation key"@en-AU ;
    skos:narrower F2021L00313:304 ;
    skos:prefLabel "Item I306"@en-AU ;
    dcat:accessURL <https://www.legislation.gov.au/F2021L00313/2023-08-04/2023-08-04/text/original/epub/OEBPS/document_1/document_1.html#_Toc144218151> ;
    dcat:landingPage "https://www.legislation.gov.au/F2021L00313/2023-08-04/2023-08-04/text/original/epub/OEBPS/document_1/document_1.html#_Toc144218151"^^xsd:anyURI ;
    dcat:theme legcons:Item .

F2021L00313:307 a legcons:Item,
        owl:Class,
        dcat:Resource ;
    rdfs:label "Item - I307 Endnote 3 Legislation history"@en-AU ;
    dct:isPartOf F2021L00313:304 ;
    dct:isReferencedBy F2021L00313: ;
    rdfs:comment "Endnote 3 Legislation history - Abrievated Graph Key: I307"@en-AU ;
    skos:definition "Endnote 3 Legislation history"@en-AU ;
    skos:narrower F2021L00313:304 ;
    skos:prefLabel "Item I307"@en-AU ;
    dcat:accessURL <https://www.legislation.gov.au/F2021L00313/2023-08-04/2023-08-04/text/original/epub/OEBPS/document_1/document_1.html#_Toc144218152> ;
    dcat:landingPage "https://www.legislation.gov.au/F2021L00313/2023-08-04/2023-08-04/text/original/epub/OEBPS/document_1/document_1.html#_Toc144218152"^^xsd:anyURI ;
    dcat:theme legcons:Item .

F2021L00313:308 a legcons:Item,
        owl:Class,
        dcat:Resource ;
    rdfs:label "Item - I308 Endnote 4 Amendment history"@en-AU ;
    dct:isPartOf F2021L00313:304 ;
    dct:isReferencedBy F2021L00313: ;
    rdfs:comment "Endnote 4 Amendment history - Abrievated Graph Key: I308"@en-AU ;
    skos:definition "Endnote 4 Amendment history"@en-AU ;
    skos:narrower F2021L00313:304 ;
    skos:prefLabel "Item I308"@en-AU ;
    dcat:accessURL <https://www.legislation.gov.au/F2021L00313/2023-08-04/2023-08-04/text/original/epub/OEBPS/document_1/document_1.html#_Toc144218153> ;
    dcat:landingPage "https://www.legislation.gov.au/F2021L00313/2023-08-04/2023-08-04/text/original/epub/OEBPS/document_1/document_1.html#_Toc144218153"^^xsd:anyURI ;
    dcat:theme legcons:Item .

F2021L00313:31 a legcons:Item,
        owl:Class,
        dcat:Resource ;
    rdfs:label "Item - I31 2 11  When government certificate may be issued in relation to wild game meat or wild game meat products"@en-AU ;
    dct:isPartOf F2021L00313:30 ;
    dct:isReferencedBy F2021L00313: ;
    rdfs:comment "2 11  When government certificate may be issued in relation to wild game meat or wild game meat products - Abrievated Graph Key: I31"@en-AU ;
    skos:definition "2 11  When government certificate may be issued in relation to wild game meat or wild game meat products"@en-AU ;
    skos:narrower F2021L00313:30 ;
    skos:prefLabel "Item I31"@en-AU ;
    dcat:accessURL <https://www.legislation.gov.au/F2021L00313/2023-08-04/2023-08-04/text/original/epub/OEBPS/document_1/document_1.html#_Toc144217876> ;
    dcat:landingPage "https://www.legislation.gov.au/F2021L00313/2023-08-04/2023-08-04/text/original/epub/OEBPS/document_1/document_1.html#_Toc144217876"^^xsd:anyURI ;
    dcat:theme legcons:Item .

F2021L00313:32 a legcons:Item,
        owl:Class,
        dcat:Resource ;
    rdfs:label "Item - I32 2 12  Declaration to accompany application for government certificate"@en-AU ;
    dct:isPartOf F2021L00313:30 ;
    dct:isReferencedBy F2021L00313: ;
    rdfs:comment "2 12  Declaration to accompany application for government certificate - Abrievated Graph Key: I32"@en-AU ;
    skos:definition "2 12  Declaration to accompany application for government certificate"@en-AU ;
    skos:narrower F2021L00313:30 ;
    skos:prefLabel "Item I32"@en-AU ;
    dcat:accessURL <https://www.legislation.gov.au/F2021L00313/2023-08-04/2023-08-04/text/original/epub/OEBPS/document_1/document_1.html#_Toc144217877> ;
    dcat:landingPage "https://www.legislation.gov.au/F2021L00313/2023-08-04/2023-08-04/text/original/epub/OEBPS/document_1/document_1.html#_Toc144217877"^^xsd:anyURI ;
    dcat:theme legcons:Item .

F2021L00313:33 a legcons:Item,
        owl:Class,
        dcat:Resource ;
    rdfs:label "Item - I33 2 13  Circumstances for refusing to issue government certificate"@en-AU ;
    dct:isPartOf F2021L00313:30 ;
    dct:isReferencedBy F2021L00313: ;
    rdfs:comment "2 13  Circumstances for refusing to issue government certificate - Abrievated Graph Key: I33"@en-AU ;
    skos:definition "2 13  Circumstances for refusing to issue government certificate"@en-AU ;
    skos:narrower F2021L00313:30 ;
    skos:prefLabel "Item I33"@en-AU ;
    dcat:accessURL <https://www.legislation.gov.au/F2021L00313/2023-08-04/2023-08-04/text/original/epub/OEBPS/document_1/document_1.html#_Toc144217878> ;
    dcat:landingPage "https://www.legislation.gov.au/F2021L00313/2023-08-04/2023-08-04/text/original/epub/OEBPS/document_1/document_1.html#_Toc144217878"^^xsd:anyURI ;
    dcat:theme legcons:Item .

F2021L00313:34 a legcons:Item,
        owl:Class,
        dcat:Resource ;
    rdfs:label "Item - I34 2 14  Changes that require holder of certificate to give additional or corrected information to the issuing body"@en-AU ;
    dct:isPartOf F2021L00313:30 ;
    dct:isReferencedBy F2021L00313: ;
    rdfs:comment "2 14  Changes that require holder of certificate to give additional or corrected information to the issuing body - Abrievated Graph Key: I34"@en-AU ;
    skos:definition "2 14  Changes that require holder of certificate to give additional or corrected information to the issuing body"@en-AU ;
    skos:narrower F2021L00313:30 ;
    skos:prefLabel "Item I34"@en-AU ;
    dcat:accessURL <https://www.legislation.gov.au/F2021L00313/2023-08-04/2023-08-04/text/original/epub/OEBPS/document_1/document_1.html#_Toc144217879> ;
    dcat:landingPage "https://www.legislation.gov.au/F2021L00313/2023-08-04/2023-08-04/text/original/epub/OEBPS/document_1/document_1.html#_Toc144217879"^^xsd:anyURI ;
    dcat:theme legcons:Item .

F2021L00313:35 a legcons:Item,
        owl:Class,
        dcat:Resource ;
    rdfs:label "Item - I35 2 15  Return of government certificate"@en-AU ;
    dct:isPartOf F2021L00313:30 ;
    dct:isReferencedBy F2021L00313: ;
    rdfs:comment "2 15  Return of government certificate - Abrievated Graph Key: I35"@en-AU ;
    skos:definition "2 15  Return of government certificate"@en-AU ;
    skos:narrower F2021L00313:30 ;
    skos:prefLabel "Item I35"@en-AU ;
    dcat:accessURL <https://www.legislation.gov.au/F2021L00313/2023-08-04/2023-08-04/text/original/epub/OEBPS/document_1/document_1.html#_Toc144217880> ;
    dcat:landingPage "https://www.legislation.gov.au/F2021L00313/2023-08-04/2023-08-04/text/original/epub/OEBPS/document_1/document_1.html#_Toc144217880"^^xsd:anyURI ;
    dcat:theme legcons:Item .

F2021L00313:38 a legcons:Item,
        owl:Class,
        dcat:Resource ;
    rdfs:label "Item - I38 4 1  Purpose of this Part"@en-AU ;
    dct:isPartOf F2021L00313:37 ;
    dct:isReferencedBy F2021L00313: ;
    rdfs:comment "4 1  Purpose of this Part - Abrievated Graph Key: I38"@en-AU ;
    skos:definition "4 1  Purpose of this Part"@en-AU ;
    skos:narrower F2021L00313:37 ;
    skos:prefLabel "Item I38"@en-AU ;
    dcat:accessURL <https://www.legislation.gov.au/F2021L00313/2023-08-04/2023-08-04/text/original/epub/OEBPS/document_1/document_1.html#_Toc144217883> ;
    dcat:landingPage "https://www.legislation.gov.au/F2021L00313/2023-08-04/2023-08-04/text/original/epub/OEBPS/document_1/document_1.html#_Toc144217883"^^xsd:anyURI ;
    dcat:theme legcons:Item .

F2021L00313:39 a legcons:Item,
        owl:Class,
        dcat:Resource ;
    rdfs:label "Item - I39 4 2  Operations must be carried out in a way that will ensure requirements of the Act are complied with"@en-AU ;
    dct:isPartOf F2021L00313:37 ;
    dct:isReferencedBy F2021L00313: ;
    rdfs:comment "4 2  Operations must be carried out in a way that will ensure requirements of the Act are complied with - Abrievated Graph Key: I39"@en-AU ;
    skos:definition "4 2  Operations must be carried out in a way that will ensure requirements of the Act are complied with"@en-AU ;
    skos:narrower F2021L00313:37 ;
    skos:prefLabel "Item I39"@en-AU ;
    dcat:accessURL <https://www.legislation.gov.au/F2021L00313/2023-08-04/2023-08-04/text/original/epub/OEBPS/document_1/document_1.html#_Toc144217884> ;
    dcat:landingPage "https://www.legislation.gov.au/F2021L00313/2023-08-04/2023-08-04/text/original/epub/OEBPS/document_1/document_1.html#_Toc144217884"^^xsd:anyURI ;
    dcat:theme legcons:Item .

F2021L00313:4 a legcons:Item,
        owl:Class,
        dcat:Resource ;
    rdfs:label "Item - I4 1 3  Authority"@en-AU ;
    dct:isPartOf F2021L00313:1 ;
    dct:isReferencedBy F2021L00313: ;
    rdfs:comment "1 3  Authority - Abrievated Graph Key: I4"@en-AU ;
    skos:definition "1 3  Authority"@en-AU ;
    skos:narrower F2021L00313:1 ;
    skos:prefLabel "Item I4"@en-AU ;
    dcat:accessURL <https://www.legislation.gov.au/F2021L00313/2023-08-04/2023-08-04/text/original/epub/OEBPS/document_1/document_1.html#_Toc144217849> ;
    dcat:landingPage "https://www.legislation.gov.au/F2021L00313/2023-08-04/2023-08-04/text/original/epub/OEBPS/document_1/document_1.html#_Toc144217849"^^xsd:anyURI ;
    dcat:theme legcons:Item .

F2021L00313:40 a legcons:Item,
        owl:Class,
        dcat:Resource ;
    rdfs:label "Item - I40 4 3  Requirements of Australian Meat Standard and Australian Wild Game Meat Standard must be met"@en-AU ;
    dct:isPartOf F2021L00313:37 ;
    dct:isReferencedBy F2021L00313: ;
    rdfs:comment "4 3  Requirements of Australian Meat Standard and Australian Wild Game Meat Standard must be met - Abrievated Graph Key: I40"@en-AU ;
    skos:definition "4 3  Requirements of Australian Meat Standard and Australian Wild Game Meat Standard must be met"@en-AU ;
    skos:narrower F2021L00313:37 ;
    skos:prefLabel "Item I40"@en-AU ;
    dcat:accessURL <https://www.legislation.gov.au/F2021L00313/2023-08-04/2023-08-04/text/original/epub/OEBPS/document_1/document_1.html#_Toc144217885> ;
    dcat:landingPage "https://www.legislation.gov.au/F2021L00313/2023-08-04/2023-08-04/text/original/epub/OEBPS/document_1/document_1.html#_Toc144217885"^^xsd:anyURI ;
    dcat:theme legcons:Item .

F2021L00313:41 a legcons:Item,
        owl:Class,
        dcat:Resource ;
    rdfs:label "Item - I41 4 4  Equipment facilities and essential services"@en-AU ;
    dct:isPartOf F2021L00313:37 ;
    dct:isReferencedBy F2021L00313: ;
    rdfs:comment "4 4  Equipment facilities and essential services - Abrievated Graph Key: I41"@en-AU ;
    skos:definition "4 4  Equipment facilities and essential services"@en-AU ;
    skos:narrower F2021L00313:37 ;
    skos:prefLabel "Item I41"@en-AU ;
    dcat:accessURL <https://www.legislation.gov.au/F2021L00313/2023-08-04/2023-08-04/text/original/epub/OEBPS/document_1/document_1.html#_Toc144217886> ;
    dcat:landingPage "https://www.legislation.gov.au/F2021L00313/2023-08-04/2023-08-04/text/original/epub/OEBPS/document_1/document_1.html#_Toc144217886"^^xsd:anyURI ;
    dcat:theme legcons:Item .

F2021L00313:42 a legcons:Item,
        owl:Class,
        dcat:Resource ;
    rdfs:label "Item - I42 4 5  Areas where post mortem inspections are carried out"@en-AU ;
    dct:isPartOf F2021L00313:37 ;
    dct:isReferencedBy F2021L00313: ;
    rdfs:comment "4 5  Areas where post mortem inspections are carried out - Abrievated Graph Key: I42"@en-AU ;
    skos:definition "4 5  Areas where post mortem inspections are carried out"@en-AU ;
    skos:narrower F2021L00313:37 ;
    skos:prefLabel "Item I42"@en-AU ;
    dcat:accessURL <https://www.legislation.gov.au/F2021L00313/2023-08-04/2023-08-04/text/original/epub/OEBPS/document_1/document_1.html#_Toc144217887> ;
    dcat:landingPage "https://www.legislation.gov.au/F2021L00313/2023-08-04/2023-08-04/text/original/epub/OEBPS/document_1/document_1.html#_Toc144217887"^^xsd:anyURI ;
    dcat:theme legcons:Item .

F2021L00313:43 a legcons:Item,
        owl:Class,
        dcat:Resource ;
    rdfs:label "Item - I43 4 6  Meat examination facility"@en-AU ;
    dct:isPartOf F2021L00313:37 ;
    dct:isReferencedBy F2021L00313: ;
    rdfs:comment "4 6  Meat examination facility - Abrievated Graph Key: I43"@en-AU ;
    skos:definition "4 6  Meat examination facility"@en-AU ;
    skos:narrower F2021L00313:37 ;
    skos:prefLabel "Item I43"@en-AU ;
    dcat:accessURL <https://www.legislation.gov.au/F2021L00313/2023-08-04/2023-08-04/text/original/epub/OEBPS/document_1/document_1.html#_Toc144217888> ;
    dcat:landingPage "https://www.legislation.gov.au/F2021L00313/2023-08-04/2023-08-04/text/original/epub/OEBPS/document_1/document_1.html#_Toc144217888"^^xsd:anyURI ;
    dcat:theme legcons:Item .

F2021L00313:44 a legcons:Item,
        owl:Class,
        dcat:Resource ;
    rdfs:label "Item - I44 4 7  Secure storage area"@en-AU ;
    dct:isPartOf F2021L00313:37 ;
    dct:isReferencedBy F2021L00313: ;
    rdfs:comment "4 7  Secure storage area - Abrievated Graph Key: I44"@en-AU ;
    skos:definition "4 7  Secure storage area"@en-AU ;
    skos:narrower F2021L00313:37 ;
    skos:prefLabel "Item I44"@en-AU ;
    dcat:accessURL <https://www.legislation.gov.au/F2021L00313/2023-08-04/2023-08-04/text/original/epub/OEBPS/document_1/document_1.html#_Toc144217889> ;
    dcat:landingPage "https://www.legislation.gov.au/F2021L00313/2023-08-04/2023-08-04/text/original/epub/OEBPS/document_1/document_1.html#_Toc144217889"^^xsd:anyURI ;
    dcat:theme legcons:Item .

F2021L00313:45 a legcons:Item,
        owl:Class,
        dcat:Resource ;
    rdfs:label "Item - I45 4 8  Amenities for Commonwealth authorised officers"@en-AU ;
    dct:isPartOf F2021L00313:37 ;
    dct:isReferencedBy F2021L00313: ;
    rdfs:comment "4 8  Amenities for Commonwealth authorised officers - Abrievated Graph Key: I45"@en-AU ;
    skos:definition "4 8  Amenities for Commonwealth authorised officers"@en-AU ;
    skos:narrower F2021L00313:37 ;
    skos:prefLabel "Item I45"@en-AU ;
    dcat:accessURL <https://www.legislation.gov.au/F2021L00313/2023-08-04/2023-08-04/text/original/epub/OEBPS/document_1/document_1.html#_Toc144217890> ;
    dcat:landingPage "https://www.legislation.gov.au/F2021L00313/2023-08-04/2023-08-04/text/original/epub/OEBPS/document_1/document_1.html#_Toc144217890"^^xsd:anyURI ;
    dcat:theme legcons:Item .

F2021L00313:47 a legcons:Item,
        owl:Class,
        dcat:Resource ;
    rdfs:label "Item - I47 4 9  Purpose of this Part"@en-AU ;
    dct:isPartOf F2021L00313:46 ;
    dct:isReferencedBy F2021L00313: ;
    rdfs:comment "4 9  Purpose of this Part - Abrievated Graph Key: I47"@en-AU ;
    skos:definition "4 9  Purpose of this Part"@en-AU ;
    skos:narrower F2021L00313:46 ;
    skos:prefLabel "Item I47"@en-AU ;
    dcat:accessURL <https://www.legislation.gov.au/F2021L00313/2023-08-04/2023-08-04/text/original/epub/OEBPS/document_1/document_1.html#_Toc144217892> ;
    dcat:landingPage "https://www.legislation.gov.au/F2021L00313/2023-08-04/2023-08-04/text/original/epub/OEBPS/document_1/document_1.html#_Toc144217892"^^xsd:anyURI ;
    dcat:theme legcons:Item .

F2021L00313:48 a legcons:Item,
        owl:Class,
        dcat:Resource ;
    rdfs:label "Item - I48 4 10  Requirements for registration continue to be met"@en-AU ;
    dct:isPartOf F2021L00313:46 ;
    dct:isReferencedBy F2021L00313: ;
    rdfs:comment "4 10  Requirements for registration continue to be met - Abrievated Graph Key: I48"@en-AU ;
    skos:definition "4 10  Requirements for registration continue to be met"@en-AU ;
    skos:narrower F2021L00313:46 ;
    skos:prefLabel "Item I48"@en-AU ;
    dcat:accessURL <https://www.legislation.gov.au/F2021L00313/2023-08-04/2023-08-04/text/original/epub/OEBPS/document_1/document_1.html#_Toc144217893> ;
    dcat:landingPage "https://www.legislation.gov.au/F2021L00313/2023-08-04/2023-08-04/text/original/epub/OEBPS/document_1/document_1.html#_Toc144217893"^^xsd:anyURI ;
    dcat:theme legcons:Item .

F2021L00313:49 a legcons:Item,
        owl:Class,
        dcat:Resource ;
    rdfs:label "Item - I49 4 11  Certificate of registration must be displayed"@en-AU ;
    dct:isPartOf F2021L00313:46 ;
    dct:isReferencedBy F2021L00313: ;
    rdfs:comment "4 11  Certificate of registration must be displayed - Abrievated Graph Key: I49"@en-AU ;
    skos:definition "4 11  Certificate of registration must be displayed"@en-AU ;
    skos:narrower F2021L00313:46 ;
    skos:prefLabel "Item I49"@en-AU ;
    dcat:accessURL <https://www.legislation.gov.au/F2021L00313/2023-08-04/2023-08-04/text/original/epub/OEBPS/document_1/document_1.html#_Toc144217894> ;
    dcat:landingPage "https://www.legislation.gov.au/F2021L00313/2023-08-04/2023-08-04/text/original/epub/OEBPS/document_1/document_1.html#_Toc144217894"^^xsd:anyURI ;
    dcat:theme legcons:Item .

F2021L00313:5 a legcons:Item,
        owl:Class,
        dcat:Resource ;
    rdfs:label "Item - I5 1 4  Simplified outline of this instrument"@en-AU ;
    dct:isPartOf F2021L00313:1 ;
    dct:isReferencedBy F2021L00313: ;
    rdfs:comment "1 4  Simplified outline of this instrument - Abrievated Graph Key: I5"@en-AU ;
    skos:definition "1 4  Simplified outline of this instrument"@en-AU ;
    skos:narrower F2021L00313:1 ;
    skos:prefLabel "Item I5"@en-AU ;
    dcat:accessURL <https://www.legislation.gov.au/F2021L00313/2023-08-04/2023-08-04/text/original/epub/OEBPS/document_1/document_1.html#_Toc144217850> ;
    dcat:landingPage "https://www.legislation.gov.au/F2021L00313/2023-08-04/2023-08-04/text/original/epub/OEBPS/document_1/document_1.html#_Toc144217850"^^xsd:anyURI ;
    dcat:theme legcons:Item .

F2021L00313:50 a legcons:Item,
        owl:Class,
        dcat:Resource ;
    rdfs:label "Item - I50 4 12  Notice of certain matters must be given to persons who manage or control export operations at registered establishment"@en-AU ;
    dct:isPartOf F2021L00313:46 ;
    dct:isReferencedBy F2021L00313: ;
    rdfs:comment "4 12  Notice of certain matters must be given to persons who manage or control export operations at registered establishment - Abrievated Graph Key: I50"@en-AU ;
    skos:definition "4 12  Notice of certain matters must be given to persons who manage or control export operations at registered establishment"@en-AU ;
    skos:narrower F2021L00313:46 ;
    skos:prefLabel "Item I50"@en-AU ;
    dcat:accessURL <https://www.legislation.gov.au/F2021L00313/2023-08-04/2023-08-04/text/original/epub/OEBPS/document_1/document_1.html#_Toc144217895> ;
    dcat:landingPage "https://www.legislation.gov.au/F2021L00313/2023-08-04/2023-08-04/text/original/epub/OEBPS/document_1/document_1.html#_Toc144217895"^^xsd:anyURI ;
    dcat:theme legcons:Item .

F2021L00313:51 a legcons:Item,
        owl:Class,
        dcat:Resource ;
    rdfs:label "Item - I51 4 13  List of persons who manage or control export operations at registered establishment"@en-AU ;
    dct:isPartOf F2021L00313:46 ;
    dct:isReferencedBy F2021L00313: ;
    rdfs:comment "4 13  List of persons who manage or control export operations at registered establishment - Abrievated Graph Key: I51"@en-AU ;
    skos:definition "4 13  List of persons who manage or control export operations at registered establishment"@en-AU ;
    skos:narrower F2021L00313:46 ;
    skos:prefLabel "Item I51"@en-AU ;
    dcat:accessURL <https://www.legislation.gov.au/F2021L00313/2023-08-04/2023-08-04/text/original/epub/OEBPS/document_1/document_1.html#_Toc144217896> ;
    dcat:landingPage "https://www.legislation.gov.au/F2021L00313/2023-08-04/2023-08-04/text/original/epub/OEBPS/document_1/document_1.html#_Toc144217896"^^xsd:anyURI ;
    dcat:theme legcons:Item .

F2021L00313:52 a legcons:Item,
        owl:Class,
        dcat:Resource ;
    rdfs:label "Item - I52 4 14  Meat inspection services"@en-AU ;
    dct:isPartOf F2021L00313:46 ;
    dct:isReferencedBy F2021L00313: ;
    rdfs:comment "4 14  Meat inspection services - Abrievated Graph Key: I52"@en-AU ;
    skos:definition "4 14  Meat inspection services"@en-AU ;
    skos:narrower F2021L00313:46 ;
    skos:prefLabel "Item I52"@en-AU ;
    dcat:accessURL <https://www.legislation.gov.au/F2021L00313/2023-08-04/2023-08-04/text/original/epub/OEBPS/document_1/document_1.html#_Toc144217897> ;
    dcat:landingPage "https://www.legislation.gov.au/F2021L00313/2023-08-04/2023-08-04/text/original/epub/OEBPS/document_1/document_1.html#_Toc144217897"^^xsd:anyURI ;
    dcat:theme legcons:Item .

F2021L00313:54 a legcons:Item,
        owl:Class,
        dcat:Resource ;
    rdfs:label "Item - I54 4 15  Period within which application to renew registration must be made"@en-AU ;
    dct:isPartOf F2021L00313:53 ;
    dct:isReferencedBy F2021L00313: ;
    rdfs:comment "4 15  Period within which application to renew registration must be made - Abrievated Graph Key: I54"@en-AU ;
    skos:definition "4 15  Period within which application to renew registration must be made"@en-AU ;
    skos:narrower F2021L00313:53 ;
    skos:prefLabel "Item I54"@en-AU ;
    dcat:accessURL <https://www.legislation.gov.au/F2021L00313/2023-08-04/2023-08-04/text/original/epub/OEBPS/document_1/document_1.html#_Toc144217899> ;
    dcat:landingPage "https://www.legislation.gov.au/F2021L00313/2023-08-04/2023-08-04/text/original/epub/OEBPS/document_1/document_1.html#_Toc144217899"^^xsd:anyURI ;
    dcat:theme legcons:Item .

F2021L00313:55 a legcons:Item,
        owl:Class,
        dcat:Resource ;
    rdfs:label "Item - I55 4 16  Requirements for renewal of registration"@en-AU ;
    dct:isPartOf F2021L00313:53 ;
    dct:isReferencedBy F2021L00313: ;
    rdfs:comment "4 16  Requirements for renewal of registration - Abrievated Graph Key: I55"@en-AU ;
    skos:definition "4 16  Requirements for renewal of registration"@en-AU ;
    skos:narrower F2021L00313:53 ;
    skos:prefLabel "Item I55"@en-AU ;
    dcat:accessURL <https://www.legislation.gov.au/F2021L00313/2023-08-04/2023-08-04/text/original/epub/OEBPS/document_1/document_1.html#_Toc144217900> ;
    dcat:landingPage "https://www.legislation.gov.au/F2021L00313/2023-08-04/2023-08-04/text/original/epub/OEBPS/document_1/document_1.html#_Toc144217900"^^xsd:anyURI ;
    dcat:theme legcons:Item .

F2021L00313:57 a legcons:Item,
        owl:Class,
        dcat:Resource ;
    rdfs:label "Item - I57 4 17  Alterations for which approval is not required"@en-AU ;
    dct:isPartOf F2021L00313:56 ;
    dct:isReferencedBy F2021L00313: ;
    rdfs:comment "4 17  Alterations for which approval is not required - Abrievated Graph Key: I57"@en-AU ;
    skos:definition "4 17  Alterations for which approval is not required"@en-AU ;
    skos:narrower F2021L00313:56 ;
    skos:prefLabel "Item I57"@en-AU ;
    dcat:accessURL <https://www.legislation.gov.au/F2021L00313/2023-08-04/2023-08-04/text/original/epub/OEBPS/document_1/document_1.html#_Toc144217902> ;
    dcat:landingPage "https://www.legislation.gov.au/F2021L00313/2023-08-04/2023-08-04/text/original/epub/OEBPS/document_1/document_1.html#_Toc144217902"^^xsd:anyURI ;
    dcat:theme legcons:Item .

F2021L00313:59 a legcons:Item,
        owl:Class,
        dcat:Resource ;
    rdfs:label "Item - I59 4 18  Application of this Part"@en-AU ;
    dct:isPartOf F2021L00313:58 ;
    dct:isReferencedBy F2021L00313: ;
    rdfs:comment "4 18  Application of this Part - Abrievated Graph Key: I59"@en-AU ;
    skos:definition "4 18  Application of this Part"@en-AU ;
    skos:narrower F2021L00313:58 ;
    skos:prefLabel "Item I59"@en-AU ;
    dcat:accessURL <https://www.legislation.gov.au/F2021L00313/2023-08-04/2023-08-04/text/original/epub/OEBPS/document_1/document_1.html#_Toc144217904> ;
    dcat:landingPage "https://www.legislation.gov.au/F2021L00313/2023-08-04/2023-08-04/text/original/epub/OEBPS/document_1/document_1.html#_Toc144217904"^^xsd:anyURI ;
    dcat:theme legcons:Item .

F2021L00313:6 a legcons:Part,
        owl:Class,
        dcat:Resource ;
    rdfs:label "Part - P6 Part 2 Interpretation"@en-AU ;
    dct:isPartOf F2021L00313:1 ;
    dct:isReferencedBy F2021L00313: ;
    rdfs:comment "Part 2 Interpretation - Abrievated Graph Key: P6"@en-AU ;
    skos:definition "Part 2 Interpretation"@en-AU ;
    skos:narrower F2021L00313:1 ;
    skos:prefLabel "Part P6"@en-AU ;
    dcat:accessURL <https://www.legislation.gov.au/F2021L00313/2023-08-04/2023-08-04/text/original/epub/OEBPS/document_1/document_1.html#_Toc144217851> ;
    dcat:landingPage "https://www.legislation.gov.au/F2021L00313/2023-08-04/2023-08-04/text/original/epub/OEBPS/document_1/document_1.html#_Toc144217851"^^xsd:anyURI ;
    dcat:theme legcons:Part .

F2021L00313:60 a legcons:Item,
        owl:Class,
        dcat:Resource ;
    rdfs:label "Item - I60 4 19  Initial consideration period"@en-AU ;
    dct:isPartOf F2021L00313:58 ;
    dct:isReferencedBy F2021L00313: ;
    rdfs:comment "4 19  Initial consideration period - Abrievated Graph Key: I60"@en-AU ;
    skos:definition "4 19  Initial consideration period"@en-AU ;
    skos:narrower F2021L00313:58 ;
    skos:prefLabel "Item I60"@en-AU ;
    dcat:accessURL <https://www.legislation.gov.au/F2021L00313/2023-08-04/2023-08-04/text/original/epub/OEBPS/document_1/document_1.html#_Toc144217905> ;
    dcat:landingPage "https://www.legislation.gov.au/F2021L00313/2023-08-04/2023-08-04/text/original/epub/OEBPS/document_1/document_1.html#_Toc144217905"^^xsd:anyURI ;
    dcat:theme legcons:Item .

F2021L00313:61 a legcons:Item,
        owl:Class,
        dcat:Resource ;
    rdfs:label "Item - I61 4 20  Period within which request relating to application must be complied with"@en-AU ;
    dct:isPartOf F2021L00313:58 ;
    dct:isReferencedBy F2021L00313: ;
    rdfs:comment "4 20  Period within which request relating to application must be complied with - Abrievated Graph Key: I61"@en-AU ;
    skos:definition "4 20  Period within which request relating to application must be complied with"@en-AU ;
    skos:narrower F2021L00313:58 ;
    skos:prefLabel "Item I61"@en-AU ;
    dcat:accessURL <https://www.legislation.gov.au/F2021L00313/2023-08-04/2023-08-04/text/original/epub/OEBPS/document_1/document_1.html#_Toc144217906> ;
    dcat:landingPage "https://www.legislation.gov.au/F2021L00313/2023-08-04/2023-08-04/text/original/epub/OEBPS/document_1/document_1.html#_Toc144217906"^^xsd:anyURI ;
    dcat:theme legcons:Item .

F2021L00313:64 a legcons:Item,
        owl:Class,
        dcat:Resource ;
    rdfs:label "Item - I64 4 21  Application for allocation of meat inspection services to establishment"@en-AU ;
    dct:isPartOf F2021L00313:63 ;
    dct:isReferencedBy F2021L00313: ;
    rdfs:comment "4 21  Application for allocation of meat inspection services to establishment - Abrievated Graph Key: I64"@en-AU ;
    skos:definition "4 21  Application for allocation of meat inspection services to establishment"@en-AU ;
    skos:narrower F2021L00313:63 ;
    skos:prefLabel "Item I64"@en-AU ;
    dcat:accessURL <https://www.legislation.gov.au/F2021L00313/2023-08-04/2023-08-04/text/original/epub/OEBPS/document_1/document_1.html#_Toc144217909> ;
    dcat:landingPage "https://www.legislation.gov.au/F2021L00313/2023-08-04/2023-08-04/text/original/epub/OEBPS/document_1/document_1.html#_Toc144217909"^^xsd:anyURI ;
    dcat:theme legcons:Item .

F2021L00313:65 a legcons:Item,
        owl:Class,
        dcat:Resource ;
    rdfs:label "Item - I65 4 22  Preliminary allocation"@en-AU ;
    dct:isPartOf F2021L00313:63 ;
    dct:isReferencedBy F2021L00313: ;
    rdfs:comment "4 22  Preliminary allocation - Abrievated Graph Key: I65"@en-AU ;
    skos:definition "4 22  Preliminary allocation"@en-AU ;
    skos:narrower F2021L00313:63 ;
    skos:prefLabel "Item I65"@en-AU ;
    dcat:accessURL <https://www.legislation.gov.au/F2021L00313/2023-08-04/2023-08-04/text/original/epub/OEBPS/document_1/document_1.html#_Toc144217910> ;
    dcat:landingPage "https://www.legislation.gov.au/F2021L00313/2023-08-04/2023-08-04/text/original/epub/OEBPS/document_1/document_1.html#_Toc144217910"^^xsd:anyURI ;
    dcat:theme legcons:Item .

F2021L00313:66 a legcons:Item,
        owl:Class,
        dcat:Resource ;
    rdfs:label "Item - I66 4 23  Notice of preliminary allocation"@en-AU ;
    dct:isPartOf F2021L00313:63 ;
    dct:isReferencedBy F2021L00313: ;
    rdfs:comment "4 23  Notice of preliminary allocation - Abrievated Graph Key: I66"@en-AU ;
    skos:definition "4 23  Notice of preliminary allocation"@en-AU ;
    skos:narrower F2021L00313:63 ;
    skos:prefLabel "Item I66"@en-AU ;
    dcat:accessURL <https://www.legislation.gov.au/F2021L00313/2023-08-04/2023-08-04/text/original/epub/OEBPS/document_1/document_1.html#_Toc144217911> ;
    dcat:landingPage "https://www.legislation.gov.au/F2021L00313/2023-08-04/2023-08-04/text/original/epub/OEBPS/document_1/document_1.html#_Toc144217911"^^xsd:anyURI ;
    dcat:theme legcons:Item .

F2021L00313:67 a legcons:Item,
        owl:Class,
        dcat:Resource ;
    rdfs:label "Item - I67 4 24  Procedure following notice of preliminary allocation"@en-AU ;
    dct:isPartOf F2021L00313:63 ;
    dct:isReferencedBy F2021L00313: ;
    rdfs:comment "4 24  Procedure following notice of preliminary allocation - Abrievated Graph Key: I67"@en-AU ;
    skos:definition "4 24  Procedure following notice of preliminary allocation"@en-AU ;
    skos:narrower F2021L00313:63 ;
    skos:prefLabel "Item I67"@en-AU ;
    dcat:accessURL <https://www.legislation.gov.au/F2021L00313/2023-08-04/2023-08-04/text/original/epub/OEBPS/document_1/document_1.html#_Toc144217912> ;
    dcat:landingPage "https://www.legislation.gov.au/F2021L00313/2023-08-04/2023-08-04/text/original/epub/OEBPS/document_1/document_1.html#_Toc144217912"^^xsd:anyURI ;
    dcat:theme legcons:Item .

F2021L00313:68 a legcons:Item,
        owl:Class,
        dcat:Resource ;
    rdfs:label "Item - I68 4 25  Revised allocation"@en-AU ;
    dct:isPartOf F2021L00313:63 ;
    dct:isReferencedBy F2021L00313: ;
    rdfs:comment "4 25  Revised allocation - Abrievated Graph Key: I68"@en-AU ;
    skos:definition "4 25  Revised allocation"@en-AU ;
    skos:narrower F2021L00313:63 ;
    skos:prefLabel "Item I68"@en-AU ;
    dcat:accessURL <https://www.legislation.gov.au/F2021L00313/2023-08-04/2023-08-04/text/original/epub/OEBPS/document_1/document_1.html#_Toc144217913> ;
    dcat:landingPage "https://www.legislation.gov.au/F2021L00313/2023-08-04/2023-08-04/text/original/epub/OEBPS/document_1/document_1.html#_Toc144217913"^^xsd:anyURI ;
    dcat:theme legcons:Item .

F2021L00313:69 a legcons:Item,
        owl:Class,
        dcat:Resource ;
    rdfs:label "Item - I69 4 26  Procedure following notice of revised allocation"@en-AU ;
    dct:isPartOf F2021L00313:63 ;
    dct:isReferencedBy F2021L00313: ;
    rdfs:comment "4 26  Procedure following notice of revised allocation - Abrievated Graph Key: I69"@en-AU ;
    skos:definition "4 26  Procedure following notice of revised allocation"@en-AU ;
    skos:narrower F2021L00313:63 ;
    skos:prefLabel "Item I69"@en-AU ;
    dcat:accessURL <https://www.legislation.gov.au/F2021L00313/2023-08-04/2023-08-04/text/original/epub/OEBPS/document_1/document_1.html#_Toc144217914> ;
    dcat:landingPage "https://www.legislation.gov.au/F2021L00313/2023-08-04/2023-08-04/text/original/epub/OEBPS/document_1/document_1.html#_Toc144217914"^^xsd:anyURI ;
    dcat:theme legcons:Item .

F2021L00313:7 a legcons:Division,
        owl:Class,
        dcat:Resource ;
    rdfs:label "Division - D7 Division 1 Definitions"@en-AU ;
    dct:isPartOf F2021L00313:1 ;
    dct:isReferencedBy F2021L00313: ;
    rdfs:comment "Division 1 Definitions - Abrievated Graph Key: D7"@en-AU ;
    skos:definition "Division 1 Definitions"@en-AU ;
    skos:narrower F2021L00313:1 ;
    skos:prefLabel "Division D7"@en-AU ;
    dcat:accessURL <https://www.legislation.gov.au/F2021L00313/2023-08-04/2023-08-04/text/original/epub/OEBPS/document_1/document_1.html#_Toc144217852> ;
    dcat:landingPage "https://www.legislation.gov.au/F2021L00313/2023-08-04/2023-08-04/text/original/epub/OEBPS/document_1/document_1.html#_Toc144217852"^^xsd:anyURI ;
    dcat:theme legcons:Division .

F2021L00313:70 a legcons:Item,
        owl:Class,
        dcat:Resource ;
    rdfs:label "Item - I70 4 27  Review of Secretarys determination"@en-AU ;
    dct:isPartOf F2021L00313:63 ;
    dct:isReferencedBy F2021L00313: ;
    rdfs:comment "4 27  Review of Secretarys determination - Abrievated Graph Key: I70"@en-AU ;
    skos:definition "4 27  Review of Secretarys determination"@en-AU ;
    skos:narrower F2021L00313:63 ;
    skos:prefLabel "Item I70"@en-AU ;
    dcat:accessURL <https://www.legislation.gov.au/F2021L00313/2023-08-04/2023-08-04/text/original/epub/OEBPS/document_1/document_1.html#_Toc144217915> ;
    dcat:landingPage "https://www.legislation.gov.au/F2021L00313/2023-08-04/2023-08-04/text/original/epub/OEBPS/document_1/document_1.html#_Toc144217915"^^xsd:anyURI ;
    dcat:theme legcons:Item .

F2021L00313:71 a legcons:Item,
        owl:Class,
        dcat:Resource ;
    rdfs:label "Item - I71 4 28  Determination of new allocation"@en-AU ;
    dct:isPartOf F2021L00313:63 ;
    dct:isReferencedBy F2021L00313: ;
    rdfs:comment "4 28  Determination of new allocation - Abrievated Graph Key: I71"@en-AU ;
    skos:definition "4 28  Determination of new allocation"@en-AU ;
    skos:narrower F2021L00313:63 ;
    skos:prefLabel "Item I71"@en-AU ;
    dcat:accessURL <https://www.legislation.gov.au/F2021L00313/2023-08-04/2023-08-04/text/original/epub/OEBPS/document_1/document_1.html#_Toc144217916> ;
    dcat:landingPage "https://www.legislation.gov.au/F2021L00313/2023-08-04/2023-08-04/text/original/epub/OEBPS/document_1/document_1.html#_Toc144217916"^^xsd:anyURI ;
    dcat:theme legcons:Item .

F2021L00313:73 a legcons:Item,
        owl:Class,
        dcat:Resource ;
    rdfs:label "Item - I73 4 29  Application to vary allocation of meat inspection services"@en-AU ;
    dct:isPartOf F2021L00313:72 ;
    dct:isReferencedBy F2021L00313: ;
    rdfs:comment "4 29  Application to vary allocation of meat inspection services - Abrievated Graph Key: I73"@en-AU ;
    skos:definition "4 29  Application to vary allocation of meat inspection services"@en-AU ;
    skos:narrower F2021L00313:72 ;
    skos:prefLabel "Item I73"@en-AU ;
    dcat:accessURL <https://www.legislation.gov.au/F2021L00313/2023-08-04/2023-08-04/text/original/epub/OEBPS/document_1/document_1.html#_Toc144217918> ;
    dcat:landingPage "https://www.legislation.gov.au/F2021L00313/2023-08-04/2023-08-04/text/original/epub/OEBPS/document_1/document_1.html#_Toc144217918"^^xsd:anyURI ;
    dcat:theme legcons:Item .

F2021L00313:74 a legcons:Item,
        owl:Class,
        dcat:Resource ;
    rdfs:label "Item - I74 4 30  Application for additional allocation of meat inspection services"@en-AU ;
    dct:isPartOf F2021L00313:72 ;
    dct:isReferencedBy F2021L00313: ;
    rdfs:comment "4 30  Application for additional allocation of meat inspection services - Abrievated Graph Key: I74"@en-AU ;
    skos:definition "4 30  Application for additional allocation of meat inspection services"@en-AU ;
    skos:narrower F2021L00313:72 ;
    skos:prefLabel "Item I74"@en-AU ;
    dcat:accessURL <https://www.legislation.gov.au/F2021L00313/2023-08-04/2023-08-04/text/original/epub/OEBPS/document_1/document_1.html#_Toc144217919> ;
    dcat:landingPage "https://www.legislation.gov.au/F2021L00313/2023-08-04/2023-08-04/text/original/epub/OEBPS/document_1/document_1.html#_Toc144217919"^^xsd:anyURI ;
    dcat:theme legcons:Item .

F2021L00313:75 a legcons:Item,
        owl:Class,
        dcat:Resource ;
    rdfs:label "Item - I75 4 31  Notification that meat inspection services not required during shutdown period"@en-AU ;
    dct:isPartOf F2021L00313:72 ;
    dct:isReferencedBy F2021L00313: ;
    rdfs:comment "4 31  Notification that meat inspection services not required during shutdown period - Abrievated Graph Key: I75"@en-AU ;
    skos:definition "4 31  Notification that meat inspection services not required during shutdown period"@en-AU ;
    skos:narrower F2021L00313:72 ;
    skos:prefLabel "Item I75"@en-AU ;
    dcat:accessURL <https://www.legislation.gov.au/F2021L00313/2023-08-04/2023-08-04/text/original/epub/OEBPS/document_1/document_1.html#_Toc144217920> ;
    dcat:landingPage "https://www.legislation.gov.au/F2021L00313/2023-08-04/2023-08-04/text/original/epub/OEBPS/document_1/document_1.html#_Toc144217920"^^xsd:anyURI ;
    dcat:theme legcons:Item .

F2021L00313:76 a legcons:Item,
        owl:Class,
        dcat:Resource ;
    rdfs:label "Item - I76 4 32  Variation by Secretary of allocation of meat inspection services"@en-AU ;
    dct:isPartOf F2021L00313:72 ;
    dct:isReferencedBy F2021L00313: ;
    rdfs:comment "4 32  Variation by Secretary of allocation of meat inspection services - Abrievated Graph Key: I76"@en-AU ;
    skos:definition "4 32  Variation by Secretary of allocation of meat inspection services"@en-AU ;
    skos:narrower F2021L00313:72 ;
    skos:prefLabel "Item I76"@en-AU ;
    dcat:accessURL <https://www.legislation.gov.au/F2021L00313/2023-08-04/2023-08-04/text/original/epub/OEBPS/document_1/document_1.html#_Toc144217921> ;
    dcat:landingPage "https://www.legislation.gov.au/F2021L00313/2023-08-04/2023-08-04/text/original/epub/OEBPS/document_1/document_1.html#_Toc144217921"^^xsd:anyURI ;
    dcat:theme legcons:Item .

F2021L00313:77 a legcons:Item,
        owl:Class,
        dcat:Resource ;
    rdfs:label "Item - I77 4 33  Notification of termination of meat inspection services"@en-AU ;
    dct:isPartOf F2021L00313:72 ;
    dct:isReferencedBy F2021L00313: ;
    rdfs:comment "4 33  Notification of termination of meat inspection services - Abrievated Graph Key: I77"@en-AU ;
    skos:definition "4 33  Notification of termination of meat inspection services"@en-AU ;
    skos:narrower F2021L00313:72 ;
    skos:prefLabel "Item I77"@en-AU ;
    dcat:accessURL <https://www.legislation.gov.au/F2021L00313/2023-08-04/2023-08-04/text/original/epub/OEBPS/document_1/document_1.html#_Toc144217922> ;
    dcat:landingPage "https://www.legislation.gov.au/F2021L00313/2023-08-04/2023-08-04/text/original/epub/OEBPS/document_1/document_1.html#_Toc144217922"^^xsd:anyURI ;
    dcat:theme legcons:Item .

F2021L00313:8 a legcons:Item,
        owl:Class,
        dcat:Resource ;
    rdfs:label "Item - I8 1 5  Definitions"@en-AU ;
    dct:isPartOf F2021L00313:1 ;
    dct:isReferencedBy F2021L00313: ;
    rdfs:comment "1 5  Definitions - Abrievated Graph Key: I8"@en-AU ;
    skos:definition "1 5  Definitions"@en-AU ;
    skos:narrower F2021L00313:1 ;
    skos:prefLabel "Item I8"@en-AU ;
    dcat:accessURL <https://www.legislation.gov.au/F2021L00313/2023-08-04/2023-08-04/text/original/epub/OEBPS/document_1/document_1.html#_Toc144217853> ;
    dcat:landingPage "https://www.legislation.gov.au/F2021L00313/2023-08-04/2023-08-04/text/original/epub/OEBPS/document_1/document_1.html#_Toc144217853"^^xsd:anyURI ;
    dcat:theme legcons:Item .

F2021L00313:80 a legcons:Item,
        owl:Class,
        dcat:Resource ;
    rdfs:label "Item - I80 5 1  Purpose of this Part"@en-AU ;
    dct:isPartOf F2021L00313:79 ;
    dct:isReferencedBy F2021L00313: ;
    rdfs:comment "5 1  Purpose of this Part - Abrievated Graph Key: I80"@en-AU ;
    skos:definition "5 1  Purpose of this Part"@en-AU ;
    skos:narrower F2021L00313:79 ;
    skos:prefLabel "Item I80"@en-AU ;
    dcat:accessURL <https://www.legislation.gov.au/F2021L00313/2023-08-04/2023-08-04/text/original/epub/OEBPS/document_1/document_1.html#_Toc144217925> ;
    dcat:landingPage "https://www.legislation.gov.au/F2021L00313/2023-08-04/2023-08-04/text/original/epub/OEBPS/document_1/document_1.html#_Toc144217925"^^xsd:anyURI ;
    dcat:theme legcons:Item .

F2021L00313:81 a legcons:Item,
        owl:Class,
        dcat:Resource ;
    rdfs:label "Item - I81 5 2  Other requirementsproposed arrangement for operations to prepare prescribed wild game meat or wild game meat products"@en-AU ;
    dct:isPartOf F2021L00313:79 ;
    dct:isReferencedBy F2021L00313: ;
    rdfs:comment "5 2  Other requirementsproposed arrangement for operations to prepare prescribed wild game meat or wild game meat products - Abrievated Graph Key: I81"@en-AU ;
    skos:definition "5 2  Other requirementsproposed arrangement for operations to prepare prescribed wild game meat or wild game meat products"@en-AU ;
    skos:narrower F2021L00313:79 ;
    skos:prefLabel "Item I81"@en-AU ;
    dcat:accessURL <https://www.legislation.gov.au/F2021L00313/2023-08-04/2023-08-04/text/original/epub/OEBPS/document_1/document_1.html#_Toc144217926> ;
    dcat:landingPage "https://www.legislation.gov.au/F2021L00313/2023-08-04/2023-08-04/text/original/epub/OEBPS/document_1/document_1.html#_Toc144217926"^^xsd:anyURI ;
    dcat:theme legcons:Item .

F2021L00313:84 a legcons:Item,
        owl:Class,
        dcat:Resource ;
    rdfs:label "Item - I84 5 3  Purpose of this Part"@en-AU ;
    dct:isPartOf F2021L00313:83 ;
    dct:isReferencedBy F2021L00313: ;
    rdfs:comment "5 3  Purpose of this Part - Abrievated Graph Key: I84"@en-AU ;
    skos:definition "5 3  Purpose of this Part"@en-AU ;
    skos:narrower F2021L00313:83 ;
    skos:prefLabel "Item I84"@en-AU ;
    dcat:accessURL <https://www.legislation.gov.au/F2021L00313/2023-08-04/2023-08-04/text/original/epub/OEBPS/document_1/document_1.html#_Toc144217929> ;
    dcat:landingPage "https://www.legislation.gov.au/F2021L00313/2023-08-04/2023-08-04/text/original/epub/OEBPS/document_1/document_1.html#_Toc144217929"^^xsd:anyURI ;
    dcat:theme legcons:Item .

F2021L00313:86 a legcons:Item,
        owl:Class,
        dcat:Resource ;
    rdfs:label "Item - I86 5 4  Importing country requirements must be met"@en-AU ;
    dct:isPartOf F2021L00313:85 ;
    dct:isReferencedBy F2021L00313: ;
    rdfs:comment "5 4  Importing country requirements must be met - Abrievated Graph Key: I86"@en-AU ;
    skos:definition "5 4  Importing country requirements must be met"@en-AU ;
    skos:narrower F2021L00313:85 ;
    skos:prefLabel "Item I86"@en-AU ;
    dcat:accessURL <https://www.legislation.gov.au/F2021L00313/2023-08-04/2023-08-04/text/original/epub/OEBPS/document_1/document_1.html#_Toc144217931> ;
    dcat:landingPage "https://www.legislation.gov.au/F2021L00313/2023-08-04/2023-08-04/text/original/epub/OEBPS/document_1/document_1.html#_Toc144217931"^^xsd:anyURI ;
    dcat:theme legcons:Item .

F2021L00313:87 a legcons:Item,
        owl:Class,
        dcat:Resource ;
    rdfs:label "Item - I87 5 5  Requirements of Australian Meat Standard and Australian Wild Game Meat Standard must be met"@en-AU ;
    dct:isPartOf F2021L00313:85 ;
    dct:isReferencedBy F2021L00313: ;
    rdfs:comment "5 5  Requirements of Australian Meat Standard and Australian Wild Game Meat Standard must be met - Abrievated Graph Key: I87"@en-AU ;
    skos:definition "5 5  Requirements of Australian Meat Standard and Australian Wild Game Meat Standard must be met"@en-AU ;
    skos:narrower F2021L00313:85 ;
    skos:prefLabel "Item I87"@en-AU ;
    dcat:accessURL <https://www.legislation.gov.au/F2021L00313/2023-08-04/2023-08-04/text/original/epub/OEBPS/document_1/document_1.html#_Toc144217932> ;
    dcat:landingPage "https://www.legislation.gov.au/F2021L00313/2023-08-04/2023-08-04/text/original/epub/OEBPS/document_1/document_1.html#_Toc144217932"^^xsd:anyURI ;
    dcat:theme legcons:Item .

F2021L00313:89 a legcons:Item,
        owl:Class,
        dcat:Resource ;
    rdfs:label "Item - I89 5 6  Sourcing"@en-AU ;
    dct:isPartOf F2021L00313:88 ;
    dct:isReferencedBy F2021L00313: ;
    rdfs:comment "5 6  Sourcing - Abrievated Graph Key: I89"@en-AU ;
    skos:definition "5 6  Sourcing"@en-AU ;
    skos:narrower F2021L00313:88 ;
    skos:prefLabel "Item I89"@en-AU ;
    dcat:accessURL <https://www.legislation.gov.au/F2021L00313/2023-08-04/2023-08-04/text/original/epub/OEBPS/document_1/document_1.html#_Toc144217934> ;
    dcat:landingPage "https://www.legislation.gov.au/F2021L00313/2023-08-04/2023-08-04/text/original/epub/OEBPS/document_1/document_1.html#_Toc144217934"^^xsd:anyURI ;
    dcat:theme legcons:Item .

F2021L00313:9 a legcons:Item,
        owl:Class,
        dcat:Resource ;
    rdfs:label "Item - I9 1 6  Meaning of loaded for export"@en-AU ;
    dct:isPartOf F2021L00313:1 ;
    dct:isReferencedBy F2021L00313: ;
    rdfs:comment "1 6  Meaning of loaded for export - Abrievated Graph Key: I9"@en-AU ;
    skos:definition "1 6  Meaning of loaded for export"@en-AU ;
    skos:narrower F2021L00313:1 ;
    skos:prefLabel "Item I9"@en-AU ;
    dcat:accessURL <https://www.legislation.gov.au/F2021L00313/2023-08-04/2023-08-04/text/original/epub/OEBPS/document_1/document_1.html#_Toc144217854> ;
    dcat:landingPage "https://www.legislation.gov.au/F2021L00313/2023-08-04/2023-08-04/text/original/epub/OEBPS/document_1/document_1.html#_Toc144217854"^^xsd:anyURI ;
    dcat:theme legcons:Item .

F2021L00313:90 a legcons:Item,
        owl:Class,
        dcat:Resource ;
    rdfs:label "Item - I90 5 7  Harvesting chilling and transporting in the field"@en-AU ;
    dct:isPartOf F2021L00313:88 ;
    dct:isReferencedBy F2021L00313: ;
    rdfs:comment "5 7  Harvesting chilling and transporting in the field - Abrievated Graph Key: I90"@en-AU ;
    skos:definition "5 7  Harvesting chilling and transporting in the field"@en-AU ;
    skos:narrower F2021L00313:88 ;
    skos:prefLabel "Item I90"@en-AU ;
    dcat:accessURL <https://www.legislation.gov.au/F2021L00313/2023-08-04/2023-08-04/text/original/epub/OEBPS/document_1/document_1.html#_Toc144217935> ;
    dcat:landingPage "https://www.legislation.gov.au/F2021L00313/2023-08-04/2023-08-04/text/original/epub/OEBPS/document_1/document_1.html#_Toc144217935"^^xsd:anyURI ;
    dcat:theme legcons:Item .

F2021L00313:91 a legcons:Item,
        owl:Class,
        dcat:Resource ;
    rdfs:label "Item - I91 5 8  Areas where post mortem inspections are carried out"@en-AU ;
    dct:isPartOf F2021L00313:88 ;
    dct:isReferencedBy F2021L00313: ;
    rdfs:comment "5 8  Areas where post mortem inspections are carried out - Abrievated Graph Key: I91"@en-AU ;
    skos:definition "5 8  Areas where post mortem inspections are carried out"@en-AU ;
    skos:narrower F2021L00313:88 ;
    skos:prefLabel "Item I91"@en-AU ;
    dcat:accessURL <https://www.legislation.gov.au/F2021L00313/2023-08-04/2023-08-04/text/original/epub/OEBPS/document_1/document_1.html#_Toc144217936> ;
    dcat:landingPage "https://www.legislation.gov.au/F2021L00313/2023-08-04/2023-08-04/text/original/epub/OEBPS/document_1/document_1.html#_Toc144217936"^^xsd:anyURI ;
    dcat:theme legcons:Item .

F2021L00313:92 a legcons:Item,
        owl:Class,
        dcat:Resource ;
    rdfs:label "Item - I92 5 9  Compliance with dispositions"@en-AU ;
    dct:isPartOf F2021L00313:88 ;
    dct:isReferencedBy F2021L00313: ;
    rdfs:comment "5 9  Compliance with dispositions - Abrievated Graph Key: I92"@en-AU ;
    skos:definition "5 9  Compliance with dispositions"@en-AU ;
    skos:narrower F2021L00313:88 ;
    skos:prefLabel "Item I92"@en-AU ;
    dcat:accessURL <https://www.legislation.gov.au/F2021L00313/2023-08-04/2023-08-04/text/original/epub/OEBPS/document_1/document_1.html#_Toc144217937> ;
    dcat:landingPage "https://www.legislation.gov.au/F2021L00313/2023-08-04/2023-08-04/text/original/epub/OEBPS/document_1/document_1.html#_Toc144217937"^^xsd:anyURI ;
    dcat:theme legcons:Item .

F2021L00313:93 a legcons:Item,
        owl:Class,
        dcat:Resource ;
    rdfs:label "Item - I93 5 10  Loading prescribed wild game meat or wild game meat products for transfer between registered establishments"@en-AU ;
    dct:isPartOf F2021L00313:88 ;
    dct:isReferencedBy F2021L00313: ;
    rdfs:comment "5 10  Loading prescribed wild game meat or wild game meat products for transfer between registered establishments - Abrievated Graph Key: I93"@en-AU ;
    skos:definition "5 10  Loading prescribed wild game meat or wild game meat products for transfer between registered establishments"@en-AU ;
    skos:narrower F2021L00313:88 ;
    skos:prefLabel "Item I93"@en-AU ;
    dcat:accessURL <https://www.legislation.gov.au/F2021L00313/2023-08-04/2023-08-04/text/original/epub/OEBPS/document_1/document_1.html#_Toc144217938> ;
    dcat:landingPage "https://www.legislation.gov.au/F2021L00313/2023-08-04/2023-08-04/text/original/epub/OEBPS/document_1/document_1.html#_Toc144217938"^^xsd:anyURI ;
    dcat:theme legcons:Item .

F2021L00313:94 a legcons:Item,
        owl:Class,
        dcat:Resource ;
    rdfs:label "Item - I94 5 11  Loading of prescribed wild game meat or wild game meat productssupervision"@en-AU ;
    dct:isPartOf F2021L00313:88 ;
    dct:isReferencedBy F2021L00313: ;
    rdfs:comment "5 11  Loading of prescribed wild game meat or wild game meat productssupervision - Abrievated Graph Key: I94"@en-AU ;
    skos:definition "5 11  Loading of prescribed wild game meat or wild game meat productssupervision"@en-AU ;
    skos:narrower F2021L00313:88 ;
    skos:prefLabel "Item I94"@en-AU ;
    dcat:accessURL <https://www.legislation.gov.au/F2021L00313/2023-08-04/2023-08-04/text/original/epub/OEBPS/document_1/document_1.html#_Toc144217939> ;
    dcat:landingPage "https://www.legislation.gov.au/F2021L00313/2023-08-04/2023-08-04/text/original/epub/OEBPS/document_1/document_1.html#_Toc144217939"^^xsd:anyURI ;
    dcat:theme legcons:Item .

F2021L00313:95 a legcons:Item,
        owl:Class,
        dcat:Resource ;
    rdfs:label "Item - I95 5 12  Prohibitions on loading"@en-AU ;
    dct:isPartOf F2021L00313:88 ;
    dct:isReferencedBy F2021L00313: ;
    rdfs:comment "5 12  Prohibitions on loading - Abrievated Graph Key: I95"@en-AU ;
    skos:definition "5 12  Prohibitions on loading"@en-AU ;
    skos:narrower F2021L00313:88 ;
    skos:prefLabel "Item I95"@en-AU ;
    dcat:accessURL <https://www.legislation.gov.au/F2021L00313/2023-08-04/2023-08-04/text/original/epub/OEBPS/document_1/document_1.html#_Toc144217940> ;
    dcat:landingPage "https://www.legislation.gov.au/F2021L00313/2023-08-04/2023-08-04/text/original/epub/OEBPS/document_1/document_1.html#_Toc144217940"^^xsd:anyURI ;
    dcat:theme legcons:Item .

F2021L00313:96 a legcons:Item,
        owl:Class,
        dcat:Resource ;
    rdfs:label "Item - I96 5 13  Container system units and equipment for loading aircraft and vessels"@en-AU ;
    dct:isPartOf F2021L00313:88 ;
    dct:isReferencedBy F2021L00313: ;
    rdfs:comment "5 13  Container system units and equipment for loading aircraft and vessels - Abrievated Graph Key: I96"@en-AU ;
    skos:definition "5 13  Container system units and equipment for loading aircraft and vessels"@en-AU ;
    skos:narrower F2021L00313:88 ;
    skos:prefLabel "Item I96"@en-AU ;
    dcat:accessURL <https://www.legislation.gov.au/F2021L00313/2023-08-04/2023-08-04/text/original/epub/OEBPS/document_1/document_1.html#_Toc144217941> ;
    dcat:landingPage "https://www.legislation.gov.au/F2021L00313/2023-08-04/2023-08-04/text/original/epub/OEBPS/document_1/document_1.html#_Toc144217941"^^xsd:anyURI ;
    dcat:theme legcons:Item .

F2021L00313:97 a legcons:Item,
        owl:Class,
        dcat:Resource ;
    rdfs:label "Item - I97 5 14  When a bolt seal must be applied to container system unit"@en-AU ;
    dct:isPartOf F2021L00313:88 ;
    dct:isReferencedBy F2021L00313: ;
    rdfs:comment "5 14  When a bolt seal must be applied to container system unit - Abrievated Graph Key: I97"@en-AU ;
    skos:definition "5 14  When a bolt seal must be applied to container system unit"@en-AU ;
    skos:narrower F2021L00313:88 ;
    skos:prefLabel "Item I97"@en-AU ;
    dcat:accessURL <https://www.legislation.gov.au/F2021L00313/2023-08-04/2023-08-04/text/original/epub/OEBPS/document_1/document_1.html#_Toc144217942> ;
    dcat:landingPage "https://www.legislation.gov.au/F2021L00313/2023-08-04/2023-08-04/text/original/epub/OEBPS/document_1/document_1.html#_Toc144217942"^^xsd:anyURI ;
    dcat:theme legcons:Item .

F2021L00313:98 a legcons:Item,
        owl:Class,
        dcat:Resource ;
    rdfs:label "Item - I98 5 15  Transport vehicles measuring devices and other equipment"@en-AU ;
    dct:isPartOf F2021L00313:88 ;
    dct:isReferencedBy F2021L00313: ;
    rdfs:comment "5 15  Transport vehicles measuring devices and other equipment - Abrievated Graph Key: I98"@en-AU ;
    skos:definition "5 15  Transport vehicles measuring devices and other equipment"@en-AU ;
    skos:narrower F2021L00313:88 ;
    skos:prefLabel "Item I98"@en-AU ;
    dcat:accessURL <https://www.legislation.gov.au/F2021L00313/2023-08-04/2023-08-04/text/original/epub/OEBPS/document_1/document_1.html#_Toc144217943> ;
    dcat:landingPage "https://www.legislation.gov.au/F2021L00313/2023-08-04/2023-08-04/text/original/epub/OEBPS/document_1/document_1.html#_Toc144217943"^^xsd:anyURI ;
    dcat:theme legcons:Item .

F2021L00313:117 a legcons:Division,
        owl:Class,
        dcat:Resource ;
    rdfs:label "Division - D117 Division 8 Meat inspection services"@en-AU ;
    dct:hasPart F2021L00313:118 ;
    dct:isPartOf F2021L00313:82 ;
    dct:isReferencedBy F2021L00313: ;
    rdfs:comment "Division 8 Meat inspection services - Abrievated Graph Key: D117"@en-AU ;
    skos:broader F2021L00313:118 ;
    skos:definition "Division 8 Meat inspection services"@en-AU ;
    skos:narrower F2021L00313:82 ;
    skos:prefLabel "Division D117"@en-AU ;
    dcat:accessURL <https://www.legislation.gov.au/F2021L00313/2023-08-04/2023-08-04/text/original/epub/OEBPS/document_1/document_1.html#_Toc144217962> ;
    dcat:landingPage "https://www.legislation.gov.au/F2021L00313/2023-08-04/2023-08-04/text/original/epub/OEBPS/document_1/document_1.html#_Toc144217962"^^xsd:anyURI ;
    dcat:theme legcons:Division .

F2021L00313:124 a legcons:Part,
        owl:Class,
        dcat:Resource ;
    rdfs:label "Part - P124 Part 3 Renewal of approved arrangement"@en-AU ;
    dct:hasPart F2021L00313:125 ;
    dct:isPartOf F2021L00313:78 ;
    dct:isReferencedBy F2021L00313: ;
    rdfs:comment "Part 3 Renewal of approved arrangement - Abrievated Graph Key: P124"@en-AU ;
    skos:broader F2021L00313:125 ;
    skos:definition "Part 3 Renewal of approved arrangement"@en-AU ;
    skos:narrower F2021L00313:78 ;
    skos:prefLabel "Part P124"@en-AU ;
    dcat:accessURL <https://www.legislation.gov.au/F2021L00313/2023-08-04/2023-08-04/text/original/epub/OEBPS/document_1/document_1.html#_Toc144217969> ;
    dcat:landingPage "https://www.legislation.gov.au/F2021L00313/2023-08-04/2023-08-04/text/original/epub/OEBPS/document_1/document_1.html#_Toc144217969"^^xsd:anyURI ;
    dcat:theme legcons:Part .

F2021L00313:130 a legcons:Division,
        owl:Class,
        dcat:Resource ;
    rdfs:label "Division - D130 Division 2 Variations required by Secretary"@en-AU ;
    dct:hasPart F2021L00313:131 ;
    dct:isPartOf F2021L00313:126 ;
    dct:isReferencedBy F2021L00313: ;
    rdfs:comment "Division 2 Variations required by Secretary - Abrievated Graph Key: D130"@en-AU ;
    skos:broader F2021L00313:131 ;
    skos:definition "Division 2 Variations required by Secretary"@en-AU ;
    skos:narrower F2021L00313:126 ;
    skos:prefLabel "Division D130"@en-AU ;
    dcat:accessURL <https://www.legislation.gov.au/F2021L00313/2023-08-04/2023-08-04/text/original/epub/OEBPS/document_1/document_1.html#_Toc144217975> ;
    dcat:landingPage "https://www.legislation.gov.au/F2021L00313/2023-08-04/2023-08-04/text/original/epub/OEBPS/document_1/document_1.html#_Toc144217975"^^xsd:anyURI ;
    dcat:theme legcons:Division .

F2021L00313:137 a legcons:Part,
        owl:Class,
        dcat:Resource ;
    rdfs:label "Part - P137 Part 1 Issue of export permit"@en-AU ;
    dct:hasPart F2021L00313:138 ;
    dct:isPartOf F2021L00313:136 ;
    dct:isReferencedBy F2021L00313: ;
    rdfs:comment "Part 1 Issue of export permit - Abrievated Graph Key: P137"@en-AU ;
    skos:broader F2021L00313:138 ;
    skos:definition "Part 1 Issue of export permit"@en-AU ;
    skos:narrower F2021L00313:136 ;
    skos:prefLabel "Part P137"@en-AU ;
    dcat:accessURL <https://www.legislation.gov.au/F2021L00313/2023-08-04/2023-08-04/text/original/epub/OEBPS/document_1/document_1.html#_Toc144217982> ;
    dcat:landingPage "https://www.legislation.gov.au/F2021L00313/2023-08-04/2023-08-04/text/original/epub/OEBPS/document_1/document_1.html#_Toc144217982"^^xsd:anyURI ;
    dcat:theme legcons:Part .

F2021L00313:197 a legcons:Division,
        owl:Class,
        dcat:Resource ;
    rdfs:label "Division - D197 Division 1 General"@en-AU ;
    dct:hasPart F2021L00313:198 ;
    dct:isPartOf F2021L00313:196 ;
    dct:isReferencedBy F2021L00313: ;
    rdfs:comment "Division 1 General - Abrievated Graph Key: D197"@en-AU ;
    skos:broader F2021L00313:198 ;
    skos:definition "Division 1 General"@en-AU ;
    skos:narrower F2021L00313:196 ;
    skos:prefLabel "Division D197"@en-AU ;
    dcat:accessURL <https://www.legislation.gov.au/F2021L00313/2023-08-04/2023-08-04/text/original/epub/OEBPS/document_1/document_1.html#_Toc144218042> ;
    dcat:landingPage "https://www.legislation.gov.au/F2021L00313/2023-08-04/2023-08-04/text/original/epub/OEBPS/document_1/document_1.html#_Toc144218042"^^xsd:anyURI ;
    dcat:theme legcons:Division .

F2021L00313:216 a legcons:Part,
        owl:Class,
        dcat:Resource ;
    rdfs:label "Part - P216 Part 2 Assessments"@en-AU ;
    dct:hasPart F2021L00313:217 ;
    dct:isPartOf F2021L00313:195 ;
    dct:isReferencedBy F2021L00313: ;
    rdfs:comment "Part 2 Assessments - Abrievated Graph Key: P216"@en-AU ;
    skos:broader F2021L00313:217 ;
    skos:definition "Part 2 Assessments"@en-AU ;
    skos:narrower F2021L00313:195 ;
    skos:prefLabel "Part P216"@en-AU ;
    dcat:accessURL <https://www.legislation.gov.au/F2021L00313/2023-08-04/2023-08-04/text/original/epub/OEBPS/document_1/document_1.html#_Toc144218061> ;
    dcat:landingPage "https://www.legislation.gov.au/F2021L00313/2023-08-04/2023-08-04/text/original/epub/OEBPS/document_1/document_1.html#_Toc144218061"^^xsd:anyURI ;
    dcat:theme legcons:Part .

F2021L00313:218 a legcons:Part,
        owl:Class,
        dcat:Resource ;
    rdfs:label "Part - P218 Part 3 Powers of the Secretary"@en-AU ;
    dct:hasPart F2021L00313:219 ;
    dct:isPartOf F2021L00313:195 ;
    dct:isReferencedBy F2021L00313: ;
    rdfs:comment "Part 3 Powers of the Secretary - Abrievated Graph Key: P218"@en-AU ;
    skos:broader F2021L00313:219 ;
    skos:definition "Part 3 Powers of the Secretary"@en-AU ;
    skos:narrower F2021L00313:195 ;
    skos:prefLabel "Part P218"@en-AU ;
    dcat:accessURL <https://www.legislation.gov.au/F2021L00313/2023-08-04/2023-08-04/text/original/epub/OEBPS/document_1/document_1.html#_Toc144218063> ;
    dcat:landingPage "https://www.legislation.gov.au/F2021L00313/2023-08-04/2023-08-04/text/original/epub/OEBPS/document_1/document_1.html#_Toc144218063"^^xsd:anyURI ;
    dcat:theme legcons:Part .

F2021L00313:221 a legcons:Division,
        owl:Class,
        dcat:Resource ;
    rdfs:label "Division - D221 Division 1 Third party authorised officers"@en-AU ;
    dct:hasPart F2021L00313:222 ;
    dct:isPartOf F2021L00313:220 ;
    dct:isReferencedBy F2021L00313: ;
    rdfs:comment "Division 1 Third party authorised officers - Abrievated Graph Key: D221"@en-AU ;
    skos:broader F2021L00313:222 ;
    skos:definition "Division 1 Third party authorised officers"@en-AU ;
    skos:narrower F2021L00313:220 ;
    skos:prefLabel "Division D221"@en-AU ;
    dcat:accessURL <https://www.legislation.gov.au/F2021L00313/2023-08-04/2023-08-04/text/original/epub/OEBPS/document_1/document_1.html#_Toc144218066> ;
    dcat:landingPage "https://www.legislation.gov.au/F2021L00313/2023-08-04/2023-08-04/text/original/epub/OEBPS/document_1/document_1.html#_Toc144218066"^^xsd:anyURI ;
    dcat:theme legcons:Division .

F2021L00313:236 a legcons:Division,
        owl:Class,
        dcat:Resource ;
    rdfs:label "Division - D236 Division 3 Directions to deal with non compliance with the Act etc"@en-AU ;
    dct:hasPart F2021L00313:237 ;
    dct:isPartOf F2021L00313:220 ;
    dct:isReferencedBy F2021L00313: ;
    rdfs:comment "Division 3 Directions to deal with non compliance with the Act etc - Abrievated Graph Key: D236"@en-AU ;
    skos:broader F2021L00313:237 ;
    skos:definition "Division 3 Directions to deal with non compliance with the Act etc"@en-AU ;
    skos:narrower F2021L00313:220 ;
    skos:prefLabel "Division D236"@en-AU ;
    dcat:accessURL <https://www.legislation.gov.au/F2021L00313/2023-08-04/2023-08-04/text/original/epub/OEBPS/document_1/document_1.html#_Toc144218081> ;
    dcat:landingPage "https://www.legislation.gov.au/F2021L00313/2023-08-04/2023-08-04/text/original/epub/OEBPS/document_1/document_1.html#_Toc144218081"^^xsd:anyURI ;
    dcat:theme legcons:Division .

F2021L00313:238 a legcons:Division,
        owl:Class,
        dcat:Resource ;
    rdfs:label "Division - D238 Division 4 Miscellaneous"@en-AU ;
    dct:hasPart F2021L00313:239 ;
    dct:isPartOf F2021L00313:220 ;
    dct:isReferencedBy F2021L00313: ;
    rdfs:comment "Division 4 Miscellaneous - Abrievated Graph Key: D238"@en-AU ;
    skos:broader F2021L00313:239 ;
    skos:definition "Division 4 Miscellaneous"@en-AU ;
    skos:narrower F2021L00313:220 ;
    skos:prefLabel "Division D238"@en-AU ;
    dcat:accessURL <https://www.legislation.gov.au/F2021L00313/2023-08-04/2023-08-04/text/original/epub/OEBPS/document_1/document_1.html#_Toc144218083> ;
    dcat:landingPage "https://www.legislation.gov.au/F2021L00313/2023-08-04/2023-08-04/text/original/epub/OEBPS/document_1/document_1.html#_Toc144218083"^^xsd:anyURI ;
    dcat:theme legcons:Division .

F2021L00313:240 a legcons:Chapter,
        owl:Class,
        dcat:Resource ;
    rdfs:label "Chapter - C240 Chapter 10 Compliance and enforcement"@en-AU ;
    dct:hasPart F2021L00313:241,
        F2021L00313:242 ;
    dct:isReferencedBy F2021L00313: ;
    rdfs:comment "Chapter 10 Compliance and enforcement - Abrievated Graph Key: C240"@en-AU ;
    skos:broader F2021L00313:241,
        F2021L00313:242 ;
    skos:definition "Chapter 10 Compliance and enforcement"@en-AU ;
    skos:prefLabel "Chapter C240"@en-AU ;
    dcat:accessURL <https://www.legislation.gov.au/F2021L00313/2023-08-04/2023-08-04/text/original/epub/OEBPS/document_1/document_1.html#_Toc144218085> ;
    dcat:landingPage "https://www.legislation.gov.au/F2021L00313/2023-08-04/2023-08-04/text/original/epub/OEBPS/document_1/document_1.html#_Toc144218085"^^xsd:anyURI ;
    dcat:theme legcons:Chapter .

F2021L00313:244 a legcons:Part,
        owl:Class,
        dcat:Resource ;
    rdfs:label "Part - P244 Part 1 Review of decisions"@en-AU ;
    dct:hasPart F2021L00313:245 ;
    dct:isPartOf F2021L00313:243 ;
    dct:isReferencedBy F2021L00313: ;
    rdfs:comment "Part 1 Review of decisions - Abrievated Graph Key: P244"@en-AU ;
    skos:broader F2021L00313:245 ;
    skos:definition "Part 1 Review of decisions"@en-AU ;
    skos:narrower F2021L00313:243 ;
    skos:prefLabel "Part P244"@en-AU ;
    dcat:accessURL <https://www.legislation.gov.au/F2021L00313/2023-08-04/2023-08-04/text/original/epub/OEBPS/document_1/document_1.html#_Toc144218089> ;
    dcat:landingPage "https://www.legislation.gov.au/F2021L00313/2023-08-04/2023-08-04/text/original/epub/OEBPS/document_1/document_1.html#_Toc144218089"^^xsd:anyURI ;
    dcat:theme legcons:Part .

F2021L00313:257 a legcons:Part,
        owl:Class,
        dcat:Resource ;
    rdfs:label "Part - P257 Part 3 Samples"@en-AU ;
    dct:hasPart F2021L00313:258 ;
    dct:isPartOf F2021L00313:243 ;
    dct:isReferencedBy F2021L00313: ;
    rdfs:comment "Part 3 Samples - Abrievated Graph Key: P257"@en-AU ;
    skos:broader F2021L00313:258 ;
    skos:definition "Part 3 Samples"@en-AU ;
    skos:narrower F2021L00313:243 ;
    skos:prefLabel "Part P257"@en-AU ;
    dcat:accessURL <https://www.legislation.gov.au/F2021L00313/2023-08-04/2023-08-04/text/original/epub/OEBPS/document_1/document_1.html#_Toc144218102> ;
    dcat:landingPage "https://www.legislation.gov.au/F2021L00313/2023-08-04/2023-08-04/text/original/epub/OEBPS/document_1/document_1.html#_Toc144218102"^^xsd:anyURI ;
    dcat:theme legcons:Part .

F2021L00313:262 a legcons:Part,
        owl:Class,
        dcat:Resource ;
    rdfs:label "Part - P262 Part 5 Relevant Commonwealth liabilities"@en-AU ;
    dct:hasPart F2021L00313:263 ;
    dct:isPartOf F2021L00313:243 ;
    dct:isReferencedBy F2021L00313: ;
    rdfs:comment "Part 5 Relevant Commonwealth liabilities - Abrievated Graph Key: P262"@en-AU ;
    skos:broader F2021L00313:263 ;
    skos:definition "Part 5 Relevant Commonwealth liabilities"@en-AU ;
    skos:narrower F2021L00313:243 ;
    skos:prefLabel "Part P262"@en-AU ;
    dcat:accessURL <https://www.legislation.gov.au/F2021L00313/2023-08-04/2023-08-04/text/original/epub/OEBPS/document_1/document_1.html#_Toc144218107> ;
    dcat:landingPage "https://www.legislation.gov.au/F2021L00313/2023-08-04/2023-08-04/text/original/epub/OEBPS/document_1/document_1.html#_Toc144218107"^^xsd:anyURI ;
    dcat:theme legcons:Part .

F2021L00313:265 a legcons:Part,
        owl:Class,
        dcat:Resource ;
    rdfs:label "Part - P265 Part 1 Preliminary"@en-AU ;
    dct:hasPart F2021L00313:266 ;
    dct:isPartOf F2021L00313:264 ;
    dct:isReferencedBy F2021L00313: ;
    rdfs:comment "Part 1 Preliminary - Abrievated Graph Key: P265"@en-AU ;
    skos:broader F2021L00313:266 ;
    skos:definition "Part 1 Preliminary"@en-AU ;
    skos:narrower F2021L00313:264 ;
    skos:prefLabel "Part P265"@en-AU ;
    dcat:accessURL <https://www.legislation.gov.au/F2021L00313/2023-08-04/2023-08-04/text/original/epub/OEBPS/document_1/document_1.html#_Toc144218110> ;
    dcat:landingPage "https://www.legislation.gov.au/F2021L00313/2023-08-04/2023-08-04/text/original/epub/OEBPS/document_1/document_1.html#_Toc144218110"^^xsd:anyURI ;
    dcat:theme legcons:Part .

F2021L00313:285 a legcons:Part,
        owl:Class,
        dcat:Resource ;
    rdfs:label "Part - P285 Part 3 Approved arrangements"@en-AU ;
    dct:hasPart F2021L00313:286 ;
    dct:isPartOf F2021L00313:264 ;
    dct:isReferencedBy F2021L00313: ;
    rdfs:comment "Part 3 Approved arrangements - Abrievated Graph Key: P285"@en-AU ;
    skos:broader F2021L00313:286 ;
    skos:definition "Part 3 Approved arrangements"@en-AU ;
    skos:narrower F2021L00313:264 ;
    skos:prefLabel "Part P285"@en-AU ;
    dcat:accessURL <https://www.legislation.gov.au/F2021L00313/2023-08-04/2023-08-04/text/original/epub/OEBPS/document_1/document_1.html#_Toc144218130> ;
    dcat:landingPage "https://www.legislation.gov.au/F2021L00313/2023-08-04/2023-08-04/text/original/epub/OEBPS/document_1/document_1.html#_Toc144218130"^^xsd:anyURI ;
    dcat:theme legcons:Part .

F2021L00313:288 a legcons:Division,
        owl:Class,
        dcat:Resource ;
    rdfs:label "Division - D288 Division 1 Trade descriptions"@en-AU ;
    dct:hasPart F2021L00313:289 ;
    dct:isPartOf F2021L00313:287 ;
    dct:isReferencedBy F2021L00313: ;
    rdfs:comment "Division 1 Trade descriptions - Abrievated Graph Key: D288"@en-AU ;
    skos:broader F2021L00313:289 ;
    skos:definition "Division 1 Trade descriptions"@en-AU ;
    skos:narrower F2021L00313:287 ;
    skos:prefLabel "Division D288"@en-AU ;
    dcat:accessURL <https://www.legislation.gov.au/F2021L00313/2023-08-04/2023-08-04/text/original/epub/OEBPS/document_1/document_1.html#_Toc144218133> ;
    dcat:landingPage "https://www.legislation.gov.au/F2021L00313/2023-08-04/2023-08-04/text/original/epub/OEBPS/document_1/document_1.html#_Toc144218133"^^xsd:anyURI ;
    dcat:theme legcons:Division .

F2021L00313:56 a legcons:Part,
        owl:Class,
        dcat:Resource ;
    rdfs:label "Part - P56 Part 4 Variation of registration"@en-AU ;
    dct:hasPart F2021L00313:57 ;
    dct:isPartOf F2021L00313:36 ;
    dct:isReferencedBy F2021L00313: ;
    rdfs:comment "Part 4 Variation of registration - Abrievated Graph Key: P56"@en-AU ;
    skos:broader F2021L00313:57 ;
    skos:definition "Part 4 Variation of registration"@en-AU ;
    skos:narrower F2021L00313:36 ;
    skos:prefLabel "Part P56"@en-AU ;
    dcat:accessURL <https://www.legislation.gov.au/F2021L00313/2023-08-04/2023-08-04/text/original/epub/OEBPS/document_1/document_1.html#_Toc144217901> ;
    dcat:landingPage "https://www.legislation.gov.au/F2021L00313/2023-08-04/2023-08-04/text/original/epub/OEBPS/document_1/document_1.html#_Toc144217901"^^xsd:anyURI ;
    dcat:theme legcons:Part .

F2021L00313:83 a legcons:Division,
        owl:Class,
        dcat:Resource ;
    rdfs:label "Division - D83 Division 1 Purpose of this Part"@en-AU ;
    dct:hasPart F2021L00313:84 ;
    dct:isPartOf F2021L00313:82 ;
    dct:isReferencedBy F2021L00313: ;
    rdfs:comment "Division 1 Purpose of this Part - Abrievated Graph Key: D83"@en-AU ;
    skos:broader F2021L00313:84 ;
    skos:definition "Division 1 Purpose of this Part"@en-AU ;
    skos:narrower F2021L00313:82 ;
    skos:prefLabel "Division D83"@en-AU ;
    dcat:accessURL <https://www.legislation.gov.au/F2021L00313/2023-08-04/2023-08-04/text/original/epub/OEBPS/document_1/document_1.html#_Toc144217928> ;
    dcat:landingPage "https://www.legislation.gov.au/F2021L00313/2023-08-04/2023-08-04/text/original/epub/OEBPS/document_1/document_1.html#_Toc144217928"^^xsd:anyURI ;
    dcat:theme legcons:Division .

F2021L00313:114 a legcons:Division,
        owl:Class,
        dcat:Resource ;
    rdfs:label "Division - D114 Division 7 Transfers"@en-AU ;
    dct:hasPart F2021L00313:115,
        F2021L00313:116 ;
    dct:isPartOf F2021L00313:82 ;
    dct:isReferencedBy F2021L00313: ;
    rdfs:comment "Division 7 Transfers - Abrievated Graph Key: D114"@en-AU ;
    skos:broader F2021L00313:115,
        F2021L00313:116 ;
    skos:definition "Division 7 Transfers"@en-AU ;
    skos:narrower F2021L00313:82 ;
    skos:prefLabel "Division D114"@en-AU ;
    dcat:accessURL <https://www.legislation.gov.au/F2021L00313/2023-08-04/2023-08-04/text/original/epub/OEBPS/document_1/document_1.html#_Toc144217959> ;
    dcat:landingPage "https://www.legislation.gov.au/F2021L00313/2023-08-04/2023-08-04/text/original/epub/OEBPS/document_1/document_1.html#_Toc144217959"^^xsd:anyURI ;
    dcat:theme legcons:Division .

F2021L00313:126 a legcons:Part,
        owl:Class,
        dcat:Resource ;
    rdfs:label "Part - P126 Part 4 Variation of approved arrangement"@en-AU ;
    dct:hasPart F2021L00313:127,
        F2021L00313:130 ;
    dct:isPartOf F2021L00313:78 ;
    dct:isReferencedBy F2021L00313: ;
    rdfs:comment "Part 4 Variation of approved arrangement - Abrievated Graph Key: P126"@en-AU ;
    skos:broader F2021L00313:127,
        F2021L00313:130 ;
    skos:definition "Part 4 Variation of approved arrangement"@en-AU ;
    skos:narrower F2021L00313:78 ;
    skos:prefLabel "Part P126"@en-AU ;
    dcat:accessURL <https://www.legislation.gov.au/F2021L00313/2023-08-04/2023-08-04/text/original/epub/OEBPS/document_1/document_1.html#_Toc144217971> ;
    dcat:landingPage "https://www.legislation.gov.au/F2021L00313/2023-08-04/2023-08-04/text/original/epub/OEBPS/document_1/document_1.html#_Toc144217971"^^xsd:anyURI ;
    dcat:theme legcons:Part .

F2021L00313:127 a legcons:Division,
        owl:Class,
        dcat:Resource ;
    rdfs:label "Division - D127 Division 1 Variations by holder"@en-AU ;
    dct:hasPart F2021L00313:128,
        F2021L00313:129 ;
    dct:isPartOf F2021L00313:126 ;
    dct:isReferencedBy F2021L00313: ;
    rdfs:comment "Division 1 Variations by holder - Abrievated Graph Key: D127"@en-AU ;
    skos:broader F2021L00313:128,
        F2021L00313:129 ;
    skos:definition "Division 1 Variations by holder"@en-AU ;
    skos:narrower F2021L00313:126 ;
    skos:prefLabel "Division D127"@en-AU ;
    dcat:accessURL <https://www.legislation.gov.au/F2021L00313/2023-08-04/2023-08-04/text/original/epub/OEBPS/document_1/document_1.html#_Toc144217972> ;
    dcat:landingPage "https://www.legislation.gov.au/F2021L00313/2023-08-04/2023-08-04/text/original/epub/OEBPS/document_1/document_1.html#_Toc144217972"^^xsd:anyURI ;
    dcat:theme legcons:Division .

F2021L00313:136 a legcons:Chapter,
        owl:Class,
        dcat:Resource ;
    rdfs:label "Chapter - C136 Chapter 7 Export permits"@en-AU ;
    dct:hasPart F2021L00313:137,
        F2021L00313:139,
        F2021L00313:143 ;
    dct:isReferencedBy F2021L00313: ;
    rdfs:comment "Chapter 7 Export permits - Abrievated Graph Key: C136"@en-AU ;
    skos:broader F2021L00313:137,
        F2021L00313:139,
        F2021L00313:143 ;
    skos:definition "Chapter 7 Export permits"@en-AU ;
    skos:prefLabel "Chapter C136"@en-AU ;
    dcat:accessURL <https://www.legislation.gov.au/F2021L00313/2023-08-04/2023-08-04/text/original/epub/OEBPS/document_1/document_1.html#_Toc144217981> ;
    dcat:landingPage "https://www.legislation.gov.au/F2021L00313/2023-08-04/2023-08-04/text/original/epub/OEBPS/document_1/document_1.html#_Toc144217981"^^xsd:anyURI ;
    dcat:theme legcons:Chapter .

F2021L00313:148 a legcons:Chapter,
        owl:Class,
        dcat:Resource ;
    rdfs:label "Chapter - C148 Chapter 8 Other matters relating to export"@en-AU ;
    dct:hasPart F2021L00313:149,
        F2021L00313:154,
        F2021L00313:158 ;
    dct:isReferencedBy F2021L00313: ;
    rdfs:comment "Chapter 8 Other matters relating to export - Abrievated Graph Key: C148"@en-AU ;
    skos:broader F2021L00313:149,
        F2021L00313:154,
        F2021L00313:158 ;
    skos:definition "Chapter 8 Other matters relating to export"@en-AU ;
    skos:prefLabel "Chapter C148"@en-AU ;
    dcat:accessURL <https://www.legislation.gov.au/F2021L00313/2023-08-04/2023-08-04/text/original/epub/OEBPS/document_1/document_1.html#_Toc144217993> ;
    dcat:landingPage "https://www.legislation.gov.au/F2021L00313/2023-08-04/2023-08-04/text/original/epub/OEBPS/document_1/document_1.html#_Toc144217993"^^xsd:anyURI ;
    dcat:theme legcons:Chapter .

F2021L00313:15 a legcons:Chapter,
        owl:Class,
        dcat:Resource ;
    rdfs:label "Chapter - C15 Chapter 2 Exporting goods"@en-AU ;
    dct:hasPart F2021L00313:16,
        F2021L00313:23,
        F2021L00313:30 ;
    dct:isReferencedBy F2021L00313: ;
    rdfs:comment "Chapter 2 Exporting goods - Abrievated Graph Key: C15"@en-AU ;
    skos:broader F2021L00313:16,
        F2021L00313:23,
        F2021L00313:30 ;
    skos:definition "Chapter 2 Exporting goods"@en-AU ;
    skos:prefLabel "Chapter C15"@en-AU ;
    dcat:accessURL <https://www.legislation.gov.au/F2021L00313/2023-08-04/2023-08-04/text/original/epub/OEBPS/document_1/document_1.html#_Toc144217860> ;
    dcat:landingPage "https://www.legislation.gov.au/F2021L00313/2023-08-04/2023-08-04/text/original/epub/OEBPS/document_1/document_1.html#_Toc144217860"^^xsd:anyURI ;
    dcat:theme legcons:Chapter .

F2021L00313:16 a legcons:Part,
        owl:Class,
        dcat:Resource ;
    rdfs:label "Part - P16 Part 1 Goods"@en-AU ;
    dct:hasPart F2021L00313:17,
        F2021L00313:20 ;
    dct:isPartOf F2021L00313:15 ;
    dct:isReferencedBy F2021L00313: ;
    rdfs:comment "Part 1 Goods - Abrievated Graph Key: P16"@en-AU ;
    skos:broader F2021L00313:17,
        F2021L00313:20 ;
    skos:definition "Part 1 Goods"@en-AU ;
    skos:narrower F2021L00313:15 ;
    skos:prefLabel "Part P16"@en-AU ;
    dcat:accessURL <https://www.legislation.gov.au/F2021L00313/2023-08-04/2023-08-04/text/original/epub/OEBPS/document_1/document_1.html#_Toc144217861> ;
    dcat:landingPage "https://www.legislation.gov.au/F2021L00313/2023-08-04/2023-08-04/text/original/epub/OEBPS/document_1/document_1.html#_Toc144217861"^^xsd:anyURI ;
    dcat:theme legcons:Part .

F2021L00313:17 a legcons:Division,
        owl:Class,
        dcat:Resource ;
    rdfs:label "Division - D17 Division 1 Prescribed goods"@en-AU ;
    dct:hasPart F2021L00313:18,
        F2021L00313:19 ;
    dct:isPartOf F2021L00313:16 ;
    dct:isReferencedBy F2021L00313: ;
    rdfs:comment "Division 1 Prescribed goods - Abrievated Graph Key: D17"@en-AU ;
    skos:broader F2021L00313:18,
        F2021L00313:19 ;
    skos:definition "Division 1 Prescribed goods"@en-AU ;
    skos:narrower F2021L00313:16 ;
    skos:prefLabel "Division D17"@en-AU ;
    dcat:accessURL <https://www.legislation.gov.au/F2021L00313/2023-08-04/2023-08-04/text/original/epub/OEBPS/document_1/document_1.html#_Toc144217862> ;
    dcat:landingPage "https://www.legislation.gov.au/F2021L00313/2023-08-04/2023-08-04/text/original/epub/OEBPS/document_1/document_1.html#_Toc144217862"^^xsd:anyURI ;
    dcat:theme legcons:Division .

F2021L00313:20 a legcons:Division,
        owl:Class,
        dcat:Resource ;
    rdfs:label "Division - D20 Division 2 Prohibited export and prescribed export conditions"@en-AU ;
    dct:hasPart F2021L00313:21,
        F2021L00313:22 ;
    dct:isPartOf F2021L00313:16 ;
    dct:isReferencedBy F2021L00313: ;
    rdfs:comment "Division 2 Prohibited export and prescribed export conditions - Abrievated Graph Key: D20"@en-AU ;
    skos:broader F2021L00313:21,
        F2021L00313:22 ;
    skos:definition "Division 2 Prohibited export and prescribed export conditions"@en-AU ;
    skos:narrower F2021L00313:16 ;
    skos:prefLabel "Division D20"@en-AU ;
    dcat:accessURL <https://www.legislation.gov.au/F2021L00313/2023-08-04/2023-08-04/text/original/epub/OEBPS/document_1/document_1.html#_Toc144217865> ;
    dcat:landingPage "https://www.legislation.gov.au/F2021L00313/2023-08-04/2023-08-04/text/original/epub/OEBPS/document_1/document_1.html#_Toc144217865"^^xsd:anyURI ;
    dcat:theme legcons:Division .

F2021L00313:259 a legcons:Part,
        owl:Class,
        dcat:Resource ;
    rdfs:label "Part - P259 Part 4 Damaged or destroyed wild game meat or wild game meat products"@en-AU ;
    dct:hasPart F2021L00313:260,
        F2021L00313:261 ;
    dct:isPartOf F2021L00313:243 ;
    dct:isReferencedBy F2021L00313: ;
    rdfs:comment "Part 4 Damaged or destroyed wild game meat or wild game meat products - Abrievated Graph Key: P259"@en-AU ;
    skos:broader F2021L00313:260,
        F2021L00313:261 ;
    skos:definition "Part 4 Damaged or destroyed wild game meat or wild game meat products"@en-AU ;
    skos:narrower F2021L00313:243 ;
    skos:prefLabel "Part P259"@en-AU ;
    dcat:accessURL <https://www.legislation.gov.au/F2021L00313/2023-08-04/2023-08-04/text/original/epub/OEBPS/document_1/document_1.html#_Toc144218104> ;
    dcat:landingPage "https://www.legislation.gov.au/F2021L00313/2023-08-04/2023-08-04/text/original/epub/OEBPS/document_1/document_1.html#_Toc144218104"^^xsd:anyURI ;
    dcat:theme legcons:Part .

F2021L00313:290 a legcons:Division,
        owl:Class,
        dcat:Resource ;
    rdfs:label "Division - D290 Division 2 Official marks"@en-AU ;
    dct:hasPart F2021L00313:291,
        F2021L00313:292 ;
    dct:isPartOf F2021L00313:287 ;
    dct:isReferencedBy F2021L00313: ;
    rdfs:comment "Division 2 Official marks - Abrievated Graph Key: D290"@en-AU ;
    skos:broader F2021L00313:291,
        F2021L00313:292 ;
    skos:definition "Division 2 Official marks"@en-AU ;
    skos:narrower F2021L00313:287 ;
    skos:prefLabel "Division D290"@en-AU ;
    dcat:accessURL <https://www.legislation.gov.au/F2021L00313/2023-08-04/2023-08-04/text/original/epub/OEBPS/document_1/document_1.html#_Toc144218135> ;
    dcat:landingPage "https://www.legislation.gov.au/F2021L00313/2023-08-04/2023-08-04/text/original/epub/OEBPS/document_1/document_1.html#_Toc144218135"^^xsd:anyURI ;
    dcat:theme legcons:Division .

F2021L00313:293 a legcons:Division,
        owl:Class,
        dcat:Resource ;
    rdfs:label "Division - D293 Division 3 Official marking devices"@en-AU ;
    dct:hasPart F2021L00313:294,
        F2021L00313:295 ;
    dct:isPartOf F2021L00313:287 ;
    dct:isReferencedBy F2021L00313: ;
    rdfs:comment "Division 3 Official marking devices - Abrievated Graph Key: D293"@en-AU ;
    skos:broader F2021L00313:294,
        F2021L00313:295 ;
    skos:definition "Division 3 Official marking devices"@en-AU ;
    skos:narrower F2021L00313:287 ;
    skos:prefLabel "Division D293"@en-AU ;
    dcat:accessURL <https://www.legislation.gov.au/F2021L00313/2023-08-04/2023-08-04/text/original/epub/OEBPS/document_1/document_1.html#_Toc144218138> ;
    dcat:landingPage "https://www.legislation.gov.au/F2021L00313/2023-08-04/2023-08-04/text/original/epub/OEBPS/document_1/document_1.html#_Toc144218138"^^xsd:anyURI ;
    dcat:theme legcons:Division .

F2021L00313:296 a legcons:Part,
        owl:Class,
        dcat:Resource ;
    rdfs:label "Part - P296 Part 5 Powers and officials"@en-AU ;
    dct:hasPart F2021L00313:297,
        F2021L00313:301 ;
    dct:isPartOf F2021L00313:264 ;
    dct:isReferencedBy F2021L00313: ;
    rdfs:comment "Part 5 Powers and officials - Abrievated Graph Key: P296"@en-AU ;
    skos:broader F2021L00313:297,
        F2021L00313:301 ;
    skos:definition "Part 5 Powers and officials"@en-AU ;
    skos:narrower F2021L00313:264 ;
    skos:prefLabel "Part P296"@en-AU ;
    dcat:accessURL <https://www.legislation.gov.au/F2021L00313/2023-08-04/2023-08-04/text/original/epub/OEBPS/document_1/document_1.html#_Toc144218141> ;
    dcat:landingPage "https://www.legislation.gov.au/F2021L00313/2023-08-04/2023-08-04/text/original/epub/OEBPS/document_1/document_1.html#_Toc144218141"^^xsd:anyURI ;
    dcat:theme legcons:Part .

F2021L00313:301 a legcons:Division,
        owl:Class,
        dcat:Resource ;
    rdfs:label "Division - D301 Division 2 Dispositions"@en-AU ;
    dct:hasPart F2021L00313:302,
        F2021L00313:303 ;
    dct:isPartOf F2021L00313:296 ;
    dct:isReferencedBy F2021L00313: ;
    rdfs:comment "Division 2 Dispositions - Abrievated Graph Key: D301"@en-AU ;
    skos:broader F2021L00313:302,
        F2021L00313:303 ;
    skos:definition "Division 2 Dispositions"@en-AU ;
    skos:narrower F2021L00313:296 ;
    skos:prefLabel "Division D301"@en-AU ;
    dcat:accessURL <https://www.legislation.gov.au/F2021L00313/2023-08-04/2023-08-04/text/original/epub/OEBPS/document_1/document_1.html#_Toc144218146> ;
    dcat:landingPage "https://www.legislation.gov.au/F2021L00313/2023-08-04/2023-08-04/text/original/epub/OEBPS/document_1/document_1.html#_Toc144218146"^^xsd:anyURI ;
    dcat:theme legcons:Division .

F2021L00313:53 a legcons:Part,
        owl:Class,
        dcat:Resource ;
    rdfs:label "Part - P53 Part 3 Renewal of registration"@en-AU ;
    dct:hasPart F2021L00313:54,
        F2021L00313:55 ;
    dct:isPartOf F2021L00313:36 ;
    dct:isReferencedBy F2021L00313: ;
    rdfs:comment "Part 3 Renewal of registration - Abrievated Graph Key: P53"@en-AU ;
    skos:broader F2021L00313:54,
        F2021L00313:55 ;
    skos:definition "Part 3 Renewal of registration"@en-AU ;
    skos:narrower F2021L00313:36 ;
    skos:prefLabel "Part P53"@en-AU ;
    dcat:accessURL <https://www.legislation.gov.au/F2021L00313/2023-08-04/2023-08-04/text/original/epub/OEBPS/document_1/document_1.html#_Toc144217898> ;
    dcat:landingPage "https://www.legislation.gov.au/F2021L00313/2023-08-04/2023-08-04/text/original/epub/OEBPS/document_1/document_1.html#_Toc144217898"^^xsd:anyURI ;
    dcat:theme legcons:Part .

F2021L00313:62 a legcons:Part,
        owl:Class,
        dcat:Resource ;
    rdfs:label "Part - P62 Part 6 Meat inspection services"@en-AU ;
    dct:hasPart F2021L00313:63,
        F2021L00313:72 ;
    dct:isPartOf F2021L00313:36 ;
    dct:isReferencedBy F2021L00313: ;
    rdfs:comment "Part 6 Meat inspection services - Abrievated Graph Key: P62"@en-AU ;
    skos:broader F2021L00313:63,
        F2021L00313:72 ;
    skos:definition "Part 6 Meat inspection services"@en-AU ;
    skos:narrower F2021L00313:36 ;
    skos:prefLabel "Part P62"@en-AU ;
    dcat:accessURL <https://www.legislation.gov.au/F2021L00313/2023-08-04/2023-08-04/text/original/epub/OEBPS/document_1/document_1.html#_Toc144217907> ;
    dcat:landingPage "https://www.legislation.gov.au/F2021L00313/2023-08-04/2023-08-04/text/original/epub/OEBPS/document_1/document_1.html#_Toc144217907"^^xsd:anyURI ;
    dcat:theme legcons:Part .

F2021L00313:79 a legcons:Part,
        owl:Class,
        dcat:Resource ;
    rdfs:label "Part - P79 Part 1 Requirements for approval"@en-AU ;
    dct:hasPart F2021L00313:80,
        F2021L00313:81 ;
    dct:isPartOf F2021L00313:78 ;
    dct:isReferencedBy F2021L00313: ;
    rdfs:comment "Part 1 Requirements for approval - Abrievated Graph Key: P79"@en-AU ;
    skos:broader F2021L00313:80,
        F2021L00313:81 ;
    skos:definition "Part 1 Requirements for approval"@en-AU ;
    skos:narrower F2021L00313:78 ;
    skos:prefLabel "Part P79"@en-AU ;
    dcat:accessURL <https://www.legislation.gov.au/F2021L00313/2023-08-04/2023-08-04/text/original/epub/OEBPS/document_1/document_1.html#_Toc144217924> ;
    dcat:landingPage "https://www.legislation.gov.au/F2021L00313/2023-08-04/2023-08-04/text/original/epub/OEBPS/document_1/document_1.html#_Toc144217924"^^xsd:anyURI ;
    dcat:theme legcons:Part .

F2021L00313:85 a legcons:Division,
        owl:Class,
        dcat:Resource ;
    rdfs:label "Division - D85 Division 2 General"@en-AU ;
    dct:hasPart F2021L00313:86,
        F2021L00313:87 ;
    dct:isPartOf F2021L00313:82 ;
    dct:isReferencedBy F2021L00313: ;
    rdfs:comment "Division 2 General - Abrievated Graph Key: D85"@en-AU ;
    skos:broader F2021L00313:86,
        F2021L00313:87 ;
    skos:definition "Division 2 General"@en-AU ;
    skos:narrower F2021L00313:82 ;
    skos:prefLabel "Division D85"@en-AU ;
    dcat:accessURL <https://www.legislation.gov.au/F2021L00313/2023-08-04/2023-08-04/text/original/epub/OEBPS/document_1/document_1.html#_Toc144217930> ;
    dcat:landingPage "https://www.legislation.gov.au/F2021L00313/2023-08-04/2023-08-04/text/original/epub/OEBPS/document_1/document_1.html#_Toc144217930"^^xsd:anyURI ;
    dcat:theme legcons:Division .

F2021L00313:99 a legcons:Division,
        owl:Class,
        dcat:Resource ;
    rdfs:label "Division - D99 Division 4 Trade descriptions"@en-AU ;
    dct:hasPart F2021L00313:100,
        F2021L00313:101 ;
    dct:isPartOf F2021L00313:82 ;
    dct:isReferencedBy F2021L00313: ;
    rdfs:comment "Division 4 Trade descriptions - Abrievated Graph Key: D99"@en-AU ;
    skos:broader F2021L00313:100,
        F2021L00313:101 ;
    skos:definition "Division 4 Trade descriptions"@en-AU ;
    skos:narrower F2021L00313:82 ;
    skos:prefLabel "Division D99"@en-AU ;
    dcat:accessURL <https://www.legislation.gov.au/F2021L00313/2023-08-04/2023-08-04/text/original/epub/OEBPS/document_1/document_1.html#_Toc144217944> ;
    dcat:landingPage "https://www.legislation.gov.au/F2021L00313/2023-08-04/2023-08-04/text/original/epub/OEBPS/document_1/document_1.html#_Toc144217944"^^xsd:anyURI ;
    dcat:theme legcons:Division .

F2021L00313:132 a legcons:Part,
        owl:Class,
        dcat:Resource ;
    rdfs:label "Part - P132 Part 5 Matters relating to applications"@en-AU ;
    dct:hasPart F2021L00313:133,
        F2021L00313:134,
        F2021L00313:135 ;
    dct:isPartOf F2021L00313:78 ;
    dct:isReferencedBy F2021L00313: ;
    rdfs:comment "Part 5 Matters relating to applications - Abrievated Graph Key: P132"@en-AU ;
    skos:broader F2021L00313:133,
        F2021L00313:134,
        F2021L00313:135 ;
    skos:definition "Part 5 Matters relating to applications"@en-AU ;
    skos:narrower F2021L00313:78 ;
    skos:prefLabel "Part P132"@en-AU ;
    dcat:accessURL <https://www.legislation.gov.au/F2021L00313/2023-08-04/2023-08-04/text/original/epub/OEBPS/document_1/document_1.html#_Toc144217977> ;
    dcat:landingPage "https://www.legislation.gov.au/F2021L00313/2023-08-04/2023-08-04/text/original/epub/OEBPS/document_1/document_1.html#_Toc144217977"^^xsd:anyURI ;
    dcat:theme legcons:Part .

F2021L00313:139 a legcons:Part,
        owl:Class,
        dcat:Resource ;
    rdfs:label "Part - P139 Part 2 Variation suspension and revocation of export permit"@en-AU ;
    dct:hasPart F2021L00313:140,
        F2021L00313:141,
        F2021L00313:142 ;
    dct:isPartOf F2021L00313:136 ;
    dct:isReferencedBy F2021L00313: ;
    rdfs:comment "Part 2 Variation suspension and revocation of export permit - Abrievated Graph Key: P139"@en-AU ;
    skos:broader F2021L00313:140,
        F2021L00313:141,
        F2021L00313:142 ;
    skos:definition "Part 2 Variation suspension and revocation of export permit"@en-AU ;
    skos:narrower F2021L00313:136 ;
    skos:prefLabel "Part P139"@en-AU ;
    dcat:accessURL <https://www.legislation.gov.au/F2021L00313/2023-08-04/2023-08-04/text/original/epub/OEBPS/document_1/document_1.html#_Toc144217984> ;
    dcat:landingPage "https://www.legislation.gov.au/F2021L00313/2023-08-04/2023-08-04/text/original/epub/OEBPS/document_1/document_1.html#_Toc144217984"^^xsd:anyURI ;
    dcat:theme legcons:Part .

F2021L00313:154 a legcons:Part,
        owl:Class,
        dcat:Resource ;
    rdfs:label "Part - P154 Part 2 Trade descriptions"@en-AU ;
    dct:hasPart F2021L00313:155,
        F2021L00313:156,
        F2021L00313:157 ;
    dct:isPartOf F2021L00313:148 ;
    dct:isReferencedBy F2021L00313: ;
    rdfs:comment "Part 2 Trade descriptions - Abrievated Graph Key: P154"@en-AU ;
    skos:broader F2021L00313:155,
        F2021L00313:156,
        F2021L00313:157 ;
    skos:definition "Part 2 Trade descriptions"@en-AU ;
    skos:narrower F2021L00313:148 ;
    skos:prefLabel "Part P154"@en-AU ;
    dcat:accessURL <https://www.legislation.gov.au/F2021L00313/2023-08-04/2023-08-04/text/original/epub/OEBPS/document_1/document_1.html#_Toc144217999> ;
    dcat:landingPage "https://www.legislation.gov.au/F2021L00313/2023-08-04/2023-08-04/text/original/epub/OEBPS/document_1/document_1.html#_Toc144217999"^^xsd:anyURI ;
    dcat:theme legcons:Part .

F2021L00313:184 a legcons:Division,
        owl:Class,
        dcat:Resource ;
    rdfs:label "Division - D184 Division 3 Marks resembling official marks"@en-AU ;
    dct:hasPart F2021L00313:185,
        F2021L00313:186,
        F2021L00313:187 ;
    dct:isPartOf F2021L00313:158 ;
    dct:isReferencedBy F2021L00313: ;
    rdfs:comment "Division 3 Marks resembling official marks - Abrievated Graph Key: D184"@en-AU ;
    skos:broader F2021L00313:185,
        F2021L00313:186,
        F2021L00313:187 ;
    skos:definition "Division 3 Marks resembling official marks"@en-AU ;
    skos:narrower F2021L00313:158 ;
    skos:prefLabel "Division D184"@en-AU ;
    dcat:accessURL <https://www.legislation.gov.au/F2021L00313/2023-08-04/2023-08-04/text/original/epub/OEBPS/document_1/document_1.html#_Toc144218029> ;
    dcat:landingPage "https://www.legislation.gov.au/F2021L00313/2023-08-04/2023-08-04/text/original/epub/OEBPS/document_1/document_1.html#_Toc144218029"^^xsd:anyURI ;
    dcat:theme legcons:Division .

F2021L00313:195 a legcons:Chapter,
        owl:Class,
        dcat:Resource ;
    rdfs:label "Chapter - C195 Chapter 9 Powers and officials"@en-AU ;
    dct:hasPart F2021L00313:196,
        F2021L00313:216,
        F2021L00313:218,
        F2021L00313:220 ;
    dct:isReferencedBy F2021L00313: ;
    rdfs:comment "Chapter 9 Powers and officials - Abrievated Graph Key: C195"@en-AU ;
    skos:broader F2021L00313:196,
        F2021L00313:216,
        F2021L00313:218,
        F2021L00313:220 ;
    skos:definition "Chapter 9 Powers and officials"@en-AU ;
    skos:prefLabel "Chapter C195"@en-AU ;
    dcat:accessURL <https://www.legislation.gov.au/F2021L00313/2023-08-04/2023-08-04/text/original/epub/OEBPS/document_1/document_1.html#_Toc144218040> ;
    dcat:landingPage "https://www.legislation.gov.au/F2021L00313/2023-08-04/2023-08-04/text/original/epub/OEBPS/document_1/document_1.html#_Toc144218040"^^xsd:anyURI ;
    dcat:theme legcons:Chapter .

F2021L00313:196 a legcons:Part,
        owl:Class,
        dcat:Resource ;
    rdfs:label "Part - P196 Part 1 Audits"@en-AU ;
    dct:hasPart F2021L00313:197,
        F2021L00313:199,
        F2021L00313:204 ;
    dct:isPartOf F2021L00313:195 ;
    dct:isReferencedBy F2021L00313: ;
    rdfs:comment "Part 1 Audits - Abrievated Graph Key: P196"@en-AU ;
    skos:broader F2021L00313:197,
        F2021L00313:199,
        F2021L00313:204 ;
    skos:definition "Part 1 Audits"@en-AU ;
    skos:narrower F2021L00313:195 ;
    skos:prefLabel "Part P196"@en-AU ;
    dcat:accessURL <https://www.legislation.gov.au/F2021L00313/2023-08-04/2023-08-04/text/original/epub/OEBPS/document_1/document_1.html#_Toc144218041> ;
    dcat:landingPage "https://www.legislation.gov.au/F2021L00313/2023-08-04/2023-08-04/text/original/epub/OEBPS/document_1/document_1.html#_Toc144218041"^^xsd:anyURI ;
    dcat:theme legcons:Part .

F2021L00313:287 a legcons:Part,
        owl:Class,
        dcat:Resource ;
    rdfs:label "Part - P287 Part 4 Other matters relating to export"@en-AU ;
    dct:hasPart F2021L00313:288,
        F2021L00313:290,
        F2021L00313:293 ;
    dct:isPartOf F2021L00313:264 ;
    dct:isReferencedBy F2021L00313: ;
    rdfs:comment "Part 4 Other matters relating to export - Abrievated Graph Key: P287"@en-AU ;
    skos:broader F2021L00313:288,
        F2021L00313:290,
        F2021L00313:293 ;
    skos:definition "Part 4 Other matters relating to export"@en-AU ;
    skos:narrower F2021L00313:264 ;
    skos:prefLabel "Part P287"@en-AU ;
    dcat:accessURL <https://www.legislation.gov.au/F2021L00313/2023-08-04/2023-08-04/text/original/epub/OEBPS/document_1/document_1.html#_Toc144218132> ;
    dcat:landingPage "https://www.legislation.gov.au/F2021L00313/2023-08-04/2023-08-04/text/original/epub/OEBPS/document_1/document_1.html#_Toc144218132"^^xsd:anyURI ;
    dcat:theme legcons:Part .

F2021L00313:297 a legcons:Division,
        owl:Class,
        dcat:Resource ;
    rdfs:label "Division - D297 Division 1 Approved auditors"@en-AU ;
    dct:hasPart F2021L00313:298,
        F2021L00313:299,
        F2021L00313:300 ;
    dct:isPartOf F2021L00313:296 ;
    dct:isReferencedBy F2021L00313: ;
    rdfs:comment "Division 1 Approved auditors - Abrievated Graph Key: D297"@en-AU ;
    skos:broader F2021L00313:298,
        F2021L00313:299,
        F2021L00313:300 ;
    skos:definition "Division 1 Approved auditors"@en-AU ;
    skos:narrower F2021L00313:296 ;
    skos:prefLabel "Division D297"@en-AU ;
    dcat:accessURL <https://www.legislation.gov.au/F2021L00313/2023-08-04/2023-08-04/text/original/epub/OEBPS/document_1/document_1.html#_Toc144218142> ;
    dcat:landingPage "https://www.legislation.gov.au/F2021L00313/2023-08-04/2023-08-04/text/original/epub/OEBPS/document_1/document_1.html#_Toc144218142"^^xsd:anyURI ;
    dcat:theme legcons:Division .

F2021L00313:58 a legcons:Part,
        owl:Class,
        dcat:Resource ;
    rdfs:label "Part - P58 Part 5 Matters relating to applications"@en-AU ;
    dct:hasPart F2021L00313:59,
        F2021L00313:60,
        F2021L00313:61 ;
    dct:isPartOf F2021L00313:36 ;
    dct:isReferencedBy F2021L00313: ;
    rdfs:comment "Part 5 Matters relating to applications - Abrievated Graph Key: P58"@en-AU ;
    skos:broader F2021L00313:59,
        F2021L00313:60,
        F2021L00313:61 ;
    skos:definition "Part 5 Matters relating to applications"@en-AU ;
    skos:narrower F2021L00313:36 ;
    skos:prefLabel "Part P58"@en-AU ;
    dcat:accessURL <https://www.legislation.gov.au/F2021L00313/2023-08-04/2023-08-04/text/original/epub/OEBPS/document_1/document_1.html#_Toc144217903> ;
    dcat:landingPage "https://www.legislation.gov.au/F2021L00313/2023-08-04/2023-08-04/text/original/epub/OEBPS/document_1/document_1.html#_Toc144217903"^^xsd:anyURI ;
    dcat:theme legcons:Part .

F2021L00313:102 a legcons:Division,
        owl:Class,
        dcat:Resource ;
    rdfs:label "Division - D102 Division 5 Official marks"@en-AU ;
    dct:hasPart F2021L00313:103,
        F2021L00313:104,
        F2021L00313:105,
        F2021L00313:106 ;
    dct:isPartOf F2021L00313:82 ;
    dct:isReferencedBy F2021L00313: ;
    rdfs:comment "Division 5 Official marks - Abrievated Graph Key: D102"@en-AU ;
    skos:broader F2021L00313:103,
        F2021L00313:104,
        F2021L00313:105,
        F2021L00313:106 ;
    skos:definition "Division 5 Official marks"@en-AU ;
    skos:narrower F2021L00313:82 ;
    skos:prefLabel "Division D102"@en-AU ;
    dcat:accessURL <https://www.legislation.gov.au/F2021L00313/2023-08-04/2023-08-04/text/original/epub/OEBPS/document_1/document_1.html#_Toc144217947> ;
    dcat:landingPage "https://www.legislation.gov.au/F2021L00313/2023-08-04/2023-08-04/text/original/epub/OEBPS/document_1/document_1.html#_Toc144217947"^^xsd:anyURI ;
    dcat:theme legcons:Division .

F2021L00313:119 a legcons:Division,
        owl:Class,
        dcat:Resource ;
    rdfs:label "Division - D119 Division 9 Management practices"@en-AU ;
    dct:hasPart F2021L00313:120,
        F2021L00313:121,
        F2021L00313:122,
        F2021L00313:123 ;
    dct:isPartOf F2021L00313:82 ;
    dct:isReferencedBy F2021L00313: ;
    rdfs:comment "Division 9 Management practices - Abrievated Graph Key: D119"@en-AU ;
    skos:broader F2021L00313:120,
        F2021L00313:121,
        F2021L00313:122,
        F2021L00313:123 ;
    skos:definition "Division 9 Management practices"@en-AU ;
    skos:narrower F2021L00313:82 ;
    skos:prefLabel "Division D119"@en-AU ;
    dcat:accessURL <https://www.legislation.gov.au/F2021L00313/2023-08-04/2023-08-04/text/original/epub/OEBPS/document_1/document_1.html#_Toc144217964> ;
    dcat:landingPage "https://www.legislation.gov.au/F2021L00313/2023-08-04/2023-08-04/text/original/epub/OEBPS/document_1/document_1.html#_Toc144217964"^^xsd:anyURI ;
    dcat:theme legcons:Division .

F2021L00313:143 a legcons:Part,
        owl:Class,
        dcat:Resource ;
    rdfs:label "Part - P143 Part 3 Other matters"@en-AU ;
    dct:hasPart F2021L00313:144,
        F2021L00313:145,
        F2021L00313:146,
        F2021L00313:147 ;
    dct:isPartOf F2021L00313:136 ;
    dct:isReferencedBy F2021L00313: ;
    rdfs:comment "Part 3 Other matters - Abrievated Graph Key: P143"@en-AU ;
    skos:broader F2021L00313:144,
        F2021L00313:145,
        F2021L00313:146,
        F2021L00313:147 ;
    skos:definition "Part 3 Other matters"@en-AU ;
    skos:narrower F2021L00313:136 ;
    skos:prefLabel "Part P143"@en-AU ;
    dcat:accessURL <https://www.legislation.gov.au/F2021L00313/2023-08-04/2023-08-04/text/original/epub/OEBPS/document_1/document_1.html#_Toc144217988> ;
    dcat:landingPage "https://www.legislation.gov.au/F2021L00313/2023-08-04/2023-08-04/text/original/epub/OEBPS/document_1/document_1.html#_Toc144217988"^^xsd:anyURI ;
    dcat:theme legcons:Part .

F2021L00313:149 a legcons:Part,
        owl:Class,
        dcat:Resource ;
    rdfs:label "Part - P149 Part 1 Notices of intention to export"@en-AU ;
    dct:hasPart F2021L00313:150,
        F2021L00313:151,
        F2021L00313:152,
        F2021L00313:153 ;
    dct:isPartOf F2021L00313:148 ;
    dct:isReferencedBy F2021L00313: ;
    rdfs:comment "Part 1 Notices of intention to export - Abrievated Graph Key: P149"@en-AU ;
    skos:broader F2021L00313:150,
        F2021L00313:151,
        F2021L00313:152,
        F2021L00313:153 ;
    skos:definition "Part 1 Notices of intention to export"@en-AU ;
    skos:narrower F2021L00313:148 ;
    skos:prefLabel "Part P149"@en-AU ;
    dcat:accessURL <https://www.legislation.gov.au/F2021L00313/2023-08-04/2023-08-04/text/original/epub/OEBPS/document_1/document_1.html#_Toc144217994> ;
    dcat:landingPage "https://www.legislation.gov.au/F2021L00313/2023-08-04/2023-08-04/text/original/epub/OEBPS/document_1/document_1.html#_Toc144217994"^^xsd:anyURI ;
    dcat:theme legcons:Part .

F2021L00313:158 a legcons:Part,
        owl:Class,
        dcat:Resource ;
    rdfs:label "Part - P158 Part 3 Official marks"@en-AU ;
    dct:hasPart F2021L00313:159,
        F2021L00313:171,
        F2021L00313:184,
        F2021L00313:188 ;
    dct:isPartOf F2021L00313:148 ;
    dct:isReferencedBy F2021L00313: ;
    rdfs:comment "Part 3 Official marks - Abrievated Graph Key: P158"@en-AU ;
    skos:broader F2021L00313:159,
        F2021L00313:171,
        F2021L00313:184,
        F2021L00313:188 ;
    skos:definition "Part 3 Official marks"@en-AU ;
    skos:narrower F2021L00313:148 ;
    skos:prefLabel "Part P158"@en-AU ;
    dcat:accessURL <https://www.legislation.gov.au/F2021L00313/2023-08-04/2023-08-04/text/original/epub/OEBPS/document_1/document_1.html#_Toc144218003> ;
    dcat:landingPage "https://www.legislation.gov.au/F2021L00313/2023-08-04/2023-08-04/text/original/epub/OEBPS/document_1/document_1.html#_Toc144218003"^^xsd:anyURI ;
    dcat:theme legcons:Part .

F2021L00313:199 a legcons:Division,
        owl:Class,
        dcat:Resource ;
    rdfs:label "Division - D199 Division 2 Conduct of audit etc"@en-AU ;
    dct:hasPart F2021L00313:200,
        F2021L00313:201,
        F2021L00313:202,
        F2021L00313:203 ;
    dct:isPartOf F2021L00313:196 ;
    dct:isReferencedBy F2021L00313: ;
    rdfs:comment "Division 2 Conduct of audit etc - Abrievated Graph Key: D199"@en-AU ;
    skos:broader F2021L00313:200,
        F2021L00313:201,
        F2021L00313:202,
        F2021L00313:203 ;
    skos:definition "Division 2 Conduct of audit etc"@en-AU ;
    skos:narrower F2021L00313:196 ;
    skos:prefLabel "Division D199"@en-AU ;
    dcat:accessURL <https://www.legislation.gov.au/F2021L00313/2023-08-04/2023-08-04/text/original/epub/OEBPS/document_1/document_1.html#_Toc144218044> ;
    dcat:landingPage "https://www.legislation.gov.au/F2021L00313/2023-08-04/2023-08-04/text/original/epub/OEBPS/document_1/document_1.html#_Toc144218044"^^xsd:anyURI ;
    dcat:theme legcons:Division .

F2021L00313:220 a legcons:Part,
        owl:Class,
        dcat:Resource ;
    rdfs:label "Part - P220 Part 4 Authorised officers"@en-AU ;
    dct:hasPart F2021L00313:221,
        F2021L00313:223,
        F2021L00313:236,
        F2021L00313:238 ;
    dct:isPartOf F2021L00313:195 ;
    dct:isReferencedBy F2021L00313: ;
    rdfs:comment "Part 4 Authorised officers - Abrievated Graph Key: P220"@en-AU ;
    skos:broader F2021L00313:221,
        F2021L00313:223,
        F2021L00313:236,
        F2021L00313:238 ;
    skos:definition "Part 4 Authorised officers"@en-AU ;
    skos:narrower F2021L00313:195 ;
    skos:prefLabel "Part P220"@en-AU ;
    dcat:accessURL <https://www.legislation.gov.au/F2021L00313/2023-08-04/2023-08-04/text/original/epub/OEBPS/document_1/document_1.html#_Toc144218065> ;
    dcat:landingPage "https://www.legislation.gov.au/F2021L00313/2023-08-04/2023-08-04/text/original/epub/OEBPS/document_1/document_1.html#_Toc144218065"^^xsd:anyURI ;
    dcat:theme legcons:Part .

F2021L00313:243 a legcons:Chapter,
        owl:Class,
        dcat:Resource ;
    rdfs:label "Chapter - C243 Chapter 11 Miscellaneous"@en-AU ;
    dct:hasPart F2021L00313:244,
        F2021L00313:246,
        F2021L00313:257,
        F2021L00313:259,
        F2021L00313:262 ;
    dct:isReferencedBy F2021L00313: ;
    rdfs:comment "Chapter 11 Miscellaneous - Abrievated Graph Key: C243"@en-AU ;
    skos:broader F2021L00313:244,
        F2021L00313:246,
        F2021L00313:257,
        F2021L00313:259,
        F2021L00313:262 ;
    skos:definition "Chapter 11 Miscellaneous"@en-AU ;
    skos:prefLabel "Chapter C243"@en-AU ;
    dcat:accessURL <https://www.legislation.gov.au/F2021L00313/2023-08-04/2023-08-04/text/original/epub/OEBPS/document_1/document_1.html#_Toc144218088> ;
    dcat:landingPage "https://www.legislation.gov.au/F2021L00313/2023-08-04/2023-08-04/text/original/epub/OEBPS/document_1/document_1.html#_Toc144218088"^^xsd:anyURI ;
    dcat:theme legcons:Chapter .

F2021L00313:304 a legcons:Endnotes,
        owl:Class,
        dcat:Resource ;
    rdfs:label "Endnotes - E304 Endnotes"@en-AU ;
    dct:hasPart F2021L00313:305,
        F2021L00313:306,
        F2021L00313:307,
        F2021L00313:308 ;
    dct:isPartOf F2021L00313:264 ;
    dct:isReferencedBy F2021L00313: ;
    rdfs:comment "Endnotes - Abrievated Graph Key: E304"@en-AU ;
    skos:broader F2021L00313:305,
        F2021L00313:306,
        F2021L00313:307,
        F2021L00313:308 ;
    skos:definition "Endnotes"@en-AU ;
    skos:narrower F2021L00313:264 ;
    skos:prefLabel "Endnotes E304"@en-AU ;
    dcat:accessURL <https://www.legislation.gov.au/F2021L00313/2023-08-04/2023-08-04/text/original/epub/OEBPS/document_1/document_1.html#_Toc144218149> ;
    dcat:landingPage "https://www.legislation.gov.au/F2021L00313/2023-08-04/2023-08-04/text/original/epub/OEBPS/document_1/document_1.html#_Toc144218149"^^xsd:anyURI ;
    dcat:theme legcons:Endnotes .

F2021L00313:78 a legcons:Chapter,
        owl:Class,
        dcat:Resource ;
    rdfs:label "Chapter - C78 Chapter 5 Approved arrangements"@en-AU ;
    dct:hasPart F2021L00313:124,
        F2021L00313:126,
        F2021L00313:132,
        F2021L00313:79,
        F2021L00313:82 ;
    dct:isReferencedBy F2021L00313: ;
    rdfs:comment "Chapter 5 Approved arrangements - Abrievated Graph Key: C78"@en-AU ;
    skos:broader F2021L00313:124,
        F2021L00313:126,
        F2021L00313:132,
        F2021L00313:79,
        F2021L00313:82 ;
    skos:definition "Chapter 5 Approved arrangements"@en-AU ;
    skos:prefLabel "Chapter C78"@en-AU ;
    dcat:accessURL <https://www.legislation.gov.au/F2021L00313/2023-08-04/2023-08-04/text/original/epub/OEBPS/document_1/document_1.html#_Toc144217923> ;
    dcat:landingPage "https://www.legislation.gov.au/F2021L00313/2023-08-04/2023-08-04/text/original/epub/OEBPS/document_1/document_1.html#_Toc144217923"^^xsd:anyURI ;
    dcat:theme legcons:Chapter .

F2021L00313:264 a legcons:Chapter,
        owl:Class,
        dcat:Resource ;
    rdfs:label "Chapter - C264 Chapter 12 Transitional provisions"@en-AU ;
    dct:hasPart F2021L00313:265,
        F2021L00313:267,
        F2021L00313:285,
        F2021L00313:287,
        F2021L00313:296,
        F2021L00313:304 ;
    dct:isReferencedBy F2021L00313: ;
    rdfs:comment "Chapter 12 Transitional provisions - Abrievated Graph Key: C264"@en-AU ;
    skos:broader F2021L00313:265,
        F2021L00313:267,
        F2021L00313:285,
        F2021L00313:287,
        F2021L00313:296,
        F2021L00313:304 ;
    skos:definition "Chapter 12 Transitional provisions"@en-AU ;
    skos:prefLabel "Chapter C264"@en-AU ;
    dcat:accessURL <https://www.legislation.gov.au/F2021L00313/2023-08-04/2023-08-04/text/original/epub/OEBPS/document_1/document_1.html#_Toc144218109> ;
    dcat:landingPage "https://www.legislation.gov.au/F2021L00313/2023-08-04/2023-08-04/text/original/epub/OEBPS/document_1/document_1.html#_Toc144218109"^^xsd:anyURI ;
    dcat:theme legcons:Chapter .

F2021L00313:30 a legcons:Part,
        owl:Class,
        dcat:Resource ;
    rdfs:label "Part - P30 Part 3 Government certificates"@en-AU ;
    dct:hasPart F2021L00313:31,
        F2021L00313:32,
        F2021L00313:33,
        F2021L00313:34,
        F2021L00313:35 ;
    dct:isPartOf F2021L00313:15 ;
    dct:isReferencedBy F2021L00313: ;
    rdfs:comment "Part 3 Government certificates - Abrievated Graph Key: P30"@en-AU ;
    skos:broader F2021L00313:31,
        F2021L00313:32,
        F2021L00313:33,
        F2021L00313:34,
        F2021L00313:35 ;
    skos:definition "Part 3 Government certificates"@en-AU ;
    skos:narrower F2021L00313:15 ;
    skos:prefLabel "Part P30"@en-AU ;
    dcat:accessURL <https://www.legislation.gov.au/F2021L00313/2023-08-04/2023-08-04/text/original/epub/OEBPS/document_1/document_1.html#_Toc144217875> ;
    dcat:landingPage "https://www.legislation.gov.au/F2021L00313/2023-08-04/2023-08-04/text/original/epub/OEBPS/document_1/document_1.html#_Toc144217875"^^xsd:anyURI ;
    dcat:theme legcons:Part .

F2021L00313:36 a legcons:Chapter,
        owl:Class,
        dcat:Resource ;
    rdfs:label "Chapter - C36 Chapter 4 Registered establishments"@en-AU ;
    dct:hasPart F2021L00313:37,
        F2021L00313:46,
        F2021L00313:53,
        F2021L00313:56,
        F2021L00313:58,
        F2021L00313:62 ;
    dct:isReferencedBy F2021L00313: ;
    rdfs:comment "Chapter 4 Registered establishments - Abrievated Graph Key: C36"@en-AU ;
    skos:broader F2021L00313:37,
        F2021L00313:46,
        F2021L00313:53,
        F2021L00313:56,
        F2021L00313:58,
        F2021L00313:62 ;
    skos:definition "Chapter 4 Registered establishments"@en-AU ;
    skos:prefLabel "Chapter C36"@en-AU ;
    dcat:accessURL <https://www.legislation.gov.au/F2021L00313/2023-08-04/2023-08-04/text/original/epub/OEBPS/document_1/document_1.html#_Toc144217881> ;
    dcat:landingPage "https://www.legislation.gov.au/F2021L00313/2023-08-04/2023-08-04/text/original/epub/OEBPS/document_1/document_1.html#_Toc144217881"^^xsd:anyURI ;
    dcat:theme legcons:Chapter .

F2021L00313:72 a legcons:Division,
        owl:Class,
        dcat:Resource ;
    rdfs:label "Division - D72 Division 2 Variation of meat inspection services"@en-AU ;
    dct:hasPart F2021L00313:73,
        F2021L00313:74,
        F2021L00313:75,
        F2021L00313:76,
        F2021L00313:77 ;
    dct:isPartOf F2021L00313:62 ;
    dct:isReferencedBy F2021L00313: ;
    rdfs:comment "Division 2 Variation of meat inspection services - Abrievated Graph Key: D72"@en-AU ;
    skos:broader F2021L00313:73,
        F2021L00313:74,
        F2021L00313:75,
        F2021L00313:76,
        F2021L00313:77 ;
    skos:definition "Division 2 Variation of meat inspection services"@en-AU ;
    skos:narrower F2021L00313:62 ;
    skos:prefLabel "Division D72"@en-AU ;
    dcat:accessURL <https://www.legislation.gov.au/F2021L00313/2023-08-04/2023-08-04/text/original/epub/OEBPS/document_1/document_1.html#_Toc144217917> ;
    dcat:landingPage "https://www.legislation.gov.au/F2021L00313/2023-08-04/2023-08-04/text/original/epub/OEBPS/document_1/document_1.html#_Toc144217917"^^xsd:anyURI ;
    dcat:theme legcons:Division .

F2021L00313:107 a legcons:Division,
        owl:Class,
        dcat:Resource ;
    rdfs:label "Division - D107 Division 6 Segregation identification security traceability and integrity"@en-AU ;
    dct:hasPart F2021L00313:108,
        F2021L00313:109,
        F2021L00313:110,
        F2021L00313:111,
        F2021L00313:112,
        F2021L00313:113 ;
    dct:isPartOf F2021L00313:82 ;
    dct:isReferencedBy F2021L00313: ;
    rdfs:comment "Division 6 Segregation identification security traceability and integrity - Abrievated Graph Key: D107"@en-AU ;
    skos:broader F2021L00313:108,
        F2021L00313:109,
        F2021L00313:110,
        F2021L00313:111,
        F2021L00313:112,
        F2021L00313:113 ;
    skos:definition "Division 6 Segregation identification security traceability and integrity"@en-AU ;
    skos:narrower F2021L00313:82 ;
    skos:prefLabel "Division D107"@en-AU ;
    dcat:accessURL <https://www.legislation.gov.au/F2021L00313/2023-08-04/2023-08-04/text/original/epub/OEBPS/document_1/document_1.html#_Toc144217952> ;
    dcat:landingPage "https://www.legislation.gov.au/F2021L00313/2023-08-04/2023-08-04/text/original/epub/OEBPS/document_1/document_1.html#_Toc144217952"^^xsd:anyURI ;
    dcat:theme legcons:Division .

F2021L00313:188 a legcons:Division,
        owl:Class,
        dcat:Resource ;
    rdfs:label "Division - D188 Division 4 Official marking devices"@en-AU ;
    dct:hasPart F2021L00313:189,
        F2021L00313:190,
        F2021L00313:191,
        F2021L00313:192,
        F2021L00313:193,
        F2021L00313:194 ;
    dct:isPartOf F2021L00313:158 ;
    dct:isReferencedBy F2021L00313: ;
    rdfs:comment "Division 4 Official marking devices - Abrievated Graph Key: D188"@en-AU ;
    skos:broader F2021L00313:189,
        F2021L00313:190,
        F2021L00313:191,
        F2021L00313:192,
        F2021L00313:193,
        F2021L00313:194 ;
    skos:definition "Division 4 Official marking devices"@en-AU ;
    skos:narrower F2021L00313:158 ;
    skos:prefLabel "Division D188"@en-AU ;
    dcat:accessURL <https://www.legislation.gov.au/F2021L00313/2023-08-04/2023-08-04/text/original/epub/OEBPS/document_1/document_1.html#_Toc144218033> ;
    dcat:landingPage "https://www.legislation.gov.au/F2021L00313/2023-08-04/2023-08-04/text/original/epub/OEBPS/document_1/document_1.html#_Toc144218033"^^xsd:anyURI ;
    dcat:theme legcons:Division .

F2021L00313:23 a legcons:Part,
        owl:Class,
        dcat:Resource ;
    rdfs:label "Part - P23 Part 2 Exemptions"@en-AU ;
    dct:hasPart F2021L00313:24,
        F2021L00313:25,
        F2021L00313:26,
        F2021L00313:27,
        F2021L00313:28,
        F2021L00313:29 ;
    dct:isPartOf F2021L00313:15 ;
    dct:isReferencedBy F2021L00313: ;
    rdfs:comment "Part 2 Exemptions - Abrievated Graph Key: P23"@en-AU ;
    skos:broader F2021L00313:24,
        F2021L00313:25,
        F2021L00313:26,
        F2021L00313:27,
        F2021L00313:28,
        F2021L00313:29 ;
    skos:definition "Part 2 Exemptions"@en-AU ;
    skos:narrower F2021L00313:15 ;
    skos:prefLabel "Part P23"@en-AU ;
    dcat:accessURL <https://www.legislation.gov.au/F2021L00313/2023-08-04/2023-08-04/text/original/epub/OEBPS/document_1/document_1.html#_Toc144217868> ;
    dcat:landingPage "https://www.legislation.gov.au/F2021L00313/2023-08-04/2023-08-04/text/original/epub/OEBPS/document_1/document_1.html#_Toc144217868"^^xsd:anyURI ;
    dcat:theme legcons:Part .

F2021L00313:46 a legcons:Part,
        owl:Class,
        dcat:Resource ;
    rdfs:label "Part - P46 Part 2 Conditions of registration"@en-AU ;
    dct:hasPart F2021L00313:47,
        F2021L00313:48,
        F2021L00313:49,
        F2021L00313:50,
        F2021L00313:51,
        F2021L00313:52 ;
    dct:isPartOf F2021L00313:36 ;
    dct:isReferencedBy F2021L00313: ;
    rdfs:comment "Part 2 Conditions of registration - Abrievated Graph Key: P46"@en-AU ;
    skos:broader F2021L00313:47,
        F2021L00313:48,
        F2021L00313:49,
        F2021L00313:50,
        F2021L00313:51,
        F2021L00313:52 ;
    skos:definition "Part 2 Conditions of registration"@en-AU ;
    skos:narrower F2021L00313:36 ;
    skos:prefLabel "Part P46"@en-AU ;
    dcat:accessURL <https://www.legislation.gov.au/F2021L00313/2023-08-04/2023-08-04/text/original/epub/OEBPS/document_1/document_1.html#_Toc144217891> ;
    dcat:landingPage "https://www.legislation.gov.au/F2021L00313/2023-08-04/2023-08-04/text/original/epub/OEBPS/document_1/document_1.html#_Toc144217891"^^xsd:anyURI ;
    dcat:theme legcons:Part .

F2021L00313:37 a legcons:Part,
        owl:Class,
        dcat:Resource ;
    rdfs:label "Part - P37 Part 1 Requirements for registration"@en-AU ;
    dct:hasPart F2021L00313:38,
        F2021L00313:39,
        F2021L00313:40,
        F2021L00313:41,
        F2021L00313:42,
        F2021L00313:43,
        F2021L00313:44,
        F2021L00313:45 ;
    dct:isPartOf F2021L00313:36 ;
    dct:isReferencedBy F2021L00313: ;
    rdfs:comment "Part 1 Requirements for registration - Abrievated Graph Key: P37"@en-AU ;
    skos:broader F2021L00313:38,
        F2021L00313:39,
        F2021L00313:40,
        F2021L00313:41,
        F2021L00313:42,
        F2021L00313:43,
        F2021L00313:44,
        F2021L00313:45 ;
    skos:definition "Part 1 Requirements for registration"@en-AU ;
    skos:narrower F2021L00313:36 ;
    skos:prefLabel "Part P37"@en-AU ;
    dcat:accessURL <https://www.legislation.gov.au/F2021L00313/2023-08-04/2023-08-04/text/original/epub/OEBPS/document_1/document_1.html#_Toc144217882> ;
    dcat:landingPage "https://www.legislation.gov.au/F2021L00313/2023-08-04/2023-08-04/text/original/epub/OEBPS/document_1/document_1.html#_Toc144217882"^^xsd:anyURI ;
    dcat:theme legcons:Part .

F2021L00313:63 a legcons:Division,
        owl:Class,
        dcat:Resource ;
    rdfs:label "Division - D63 Division 1 Allocation of meat inspection services"@en-AU ;
    dct:hasPart F2021L00313:64,
        F2021L00313:65,
        F2021L00313:66,
        F2021L00313:67,
        F2021L00313:68,
        F2021L00313:69,
        F2021L00313:70,
        F2021L00313:71 ;
    dct:isPartOf F2021L00313:62 ;
    dct:isReferencedBy F2021L00313: ;
    rdfs:comment "Division 1 Allocation of meat inspection services - Abrievated Graph Key: D63"@en-AU ;
    skos:broader F2021L00313:64,
        F2021L00313:65,
        F2021L00313:66,
        F2021L00313:67,
        F2021L00313:68,
        F2021L00313:69,
        F2021L00313:70,
        F2021L00313:71 ;
    skos:definition "Division 1 Allocation of meat inspection services"@en-AU ;
    skos:narrower F2021L00313:62 ;
    skos:prefLabel "Division D63"@en-AU ;
    dcat:accessURL <https://www.legislation.gov.au/F2021L00313/2023-08-04/2023-08-04/text/original/epub/OEBPS/document_1/document_1.html#_Toc144217908> ;
    dcat:landingPage "https://www.legislation.gov.au/F2021L00313/2023-08-04/2023-08-04/text/original/epub/OEBPS/document_1/document_1.html#_Toc144217908"^^xsd:anyURI ;
    dcat:theme legcons:Division .

F2021L00313:82 a legcons:Part,
        owl:Class,
        dcat:Resource ;
    rdfs:label "Part - P82 Part 2 Conditions of approved arrangement"@en-AU ;
    dct:hasPart F2021L00313:102,
        F2021L00313:107,
        F2021L00313:114,
        F2021L00313:117,
        F2021L00313:119,
        F2021L00313:83,
        F2021L00313:85,
        F2021L00313:88,
        F2021L00313:99 ;
    dct:isPartOf F2021L00313:78 ;
    dct:isReferencedBy F2021L00313: ;
    rdfs:comment "Part 2 Conditions of approved arrangement - Abrievated Graph Key: P82"@en-AU ;
    skos:broader F2021L00313:102,
        F2021L00313:107,
        F2021L00313:114,
        F2021L00313:117,
        F2021L00313:119,
        F2021L00313:83,
        F2021L00313:85,
        F2021L00313:88,
        F2021L00313:99 ;
    skos:definition "Part 2 Conditions of approved arrangement"@en-AU ;
    skos:narrower F2021L00313:78 ;
    skos:prefLabel "Part P82"@en-AU ;
    dcat:accessURL <https://www.legislation.gov.au/F2021L00313/2023-08-04/2023-08-04/text/original/epub/OEBPS/document_1/document_1.html#_Toc144217927> ;
    dcat:landingPage "https://www.legislation.gov.au/F2021L00313/2023-08-04/2023-08-04/text/original/epub/OEBPS/document_1/document_1.html#_Toc144217927"^^xsd:anyURI ;
    dcat:theme legcons:Part .

F2021L00313:246 a legcons:Part,
        owl:Class,
        dcat:Resource ;
    rdfs:label "Part - P246 Part 2 Records"@en-AU ;
    dct:hasPart F2021L00313:247,
        F2021L00313:248,
        F2021L00313:249,
        F2021L00313:250,
        F2021L00313:251,
        F2021L00313:252,
        F2021L00313:253,
        F2021L00313:254,
        F2021L00313:255,
        F2021L00313:256 ;
    dct:isPartOf F2021L00313:243 ;
    dct:isReferencedBy F2021L00313: ;
    rdfs:comment "Part 2 Records - Abrievated Graph Key: P246"@en-AU ;
    skos:broader F2021L00313:247,
        F2021L00313:248,
        F2021L00313:249,
        F2021L00313:250,
        F2021L00313:251,
        F2021L00313:252,
        F2021L00313:253,
        F2021L00313:254,
        F2021L00313:255,
        F2021L00313:256 ;
    skos:definition "Part 2 Records"@en-AU ;
    skos:narrower F2021L00313:243 ;
    skos:prefLabel "Part P246"@en-AU ;
    dcat:accessURL <https://www.legislation.gov.au/F2021L00313/2023-08-04/2023-08-04/text/original/epub/OEBPS/document_1/document_1.html#_Toc144218091> ;
    dcat:landingPage "https://www.legislation.gov.au/F2021L00313/2023-08-04/2023-08-04/text/original/epub/OEBPS/document_1/document_1.html#_Toc144218091"^^xsd:anyURI ;
    dcat:theme legcons:Part .

F2021L00313:88 a legcons:Division,
        owl:Class,
        dcat:Resource ;
    rdfs:label "Division - D88 Division 3 Preparation and transport"@en-AU ;
    dct:hasPart F2021L00313:89,
        F2021L00313:90,
        F2021L00313:91,
        F2021L00313:92,
        F2021L00313:93,
        F2021L00313:94,
        F2021L00313:95,
        F2021L00313:96,
        F2021L00313:97,
        F2021L00313:98 ;
    dct:isPartOf F2021L00313:82 ;
    dct:isReferencedBy F2021L00313: ;
    rdfs:comment "Division 3 Preparation and transport - Abrievated Graph Key: D88"@en-AU ;
    skos:broader F2021L00313:89,
        F2021L00313:90,
        F2021L00313:91,
        F2021L00313:92,
        F2021L00313:93,
        F2021L00313:94,
        F2021L00313:95,
        F2021L00313:96,
        F2021L00313:97,
        F2021L00313:98 ;
    skos:definition "Division 3 Preparation and transport"@en-AU ;
    skos:narrower F2021L00313:82 ;
    skos:prefLabel "Division D88"@en-AU ;
    dcat:accessURL <https://www.legislation.gov.au/F2021L00313/2023-08-04/2023-08-04/text/original/epub/OEBPS/document_1/document_1.html#_Toc144217933> ;
    dcat:landingPage "https://www.legislation.gov.au/F2021L00313/2023-08-04/2023-08-04/text/original/epub/OEBPS/document_1/document_1.html#_Toc144217933"^^xsd:anyURI ;
    dcat:theme legcons:Division .

F2021L00313:159 a legcons:Division,
        owl:Class,
        dcat:Resource ;
    rdfs:label "Division - D159 Division 1 Marks that are official marks"@en-AU ;
    dct:hasPart F2021L00313:160,
        F2021L00313:161,
        F2021L00313:162,
        F2021L00313:163,
        F2021L00313:164,
        F2021L00313:165,
        F2021L00313:166,
        F2021L00313:167,
        F2021L00313:168,
        F2021L00313:169,
        F2021L00313:170 ;
    dct:isPartOf F2021L00313:158 ;
    dct:isReferencedBy F2021L00313: ;
    rdfs:comment "Division 1 Marks that are official marks - Abrievated Graph Key: D159"@en-AU ;
    skos:broader F2021L00313:160,
        F2021L00313:161,
        F2021L00313:162,
        F2021L00313:163,
        F2021L00313:164,
        F2021L00313:165,
        F2021L00313:166,
        F2021L00313:167,
        F2021L00313:168,
        F2021L00313:169,
        F2021L00313:170 ;
    skos:definition "Division 1 Marks that are official marks"@en-AU ;
    skos:narrower F2021L00313:158 ;
    skos:prefLabel "Division D159"@en-AU ;
    dcat:accessURL <https://www.legislation.gov.au/F2021L00313/2023-08-04/2023-08-04/text/original/epub/OEBPS/document_1/document_1.html#_Toc144218004> ;
    dcat:landingPage "https://www.legislation.gov.au/F2021L00313/2023-08-04/2023-08-04/text/original/epub/OEBPS/document_1/document_1.html#_Toc144218004"^^xsd:anyURI ;
    dcat:theme legcons:Division .

F2021L00313:204 a legcons:Division,
        owl:Class,
        dcat:Resource ;
    rdfs:label "Division - D204 Division 3 Approved auditors"@en-AU ;
    dct:hasPart F2021L00313:205,
        F2021L00313:206,
        F2021L00313:207,
        F2021L00313:208,
        F2021L00313:209,
        F2021L00313:210,
        F2021L00313:211,
        F2021L00313:212,
        F2021L00313:213,
        F2021L00313:214,
        F2021L00313:215 ;
    dct:isPartOf F2021L00313:196 ;
    dct:isReferencedBy F2021L00313: ;
    rdfs:comment "Division 3 Approved auditors - Abrievated Graph Key: D204"@en-AU ;
    skos:broader F2021L00313:205,
        F2021L00313:206,
        F2021L00313:207,
        F2021L00313:208,
        F2021L00313:209,
        F2021L00313:210,
        F2021L00313:211,
        F2021L00313:212,
        F2021L00313:213,
        F2021L00313:214,
        F2021L00313:215 ;
    skos:definition "Division 3 Approved auditors"@en-AU ;
    skos:narrower F2021L00313:196 ;
    skos:prefLabel "Division D204"@en-AU ;
    dcat:accessURL <https://www.legislation.gov.au/F2021L00313/2023-08-04/2023-08-04/text/original/epub/OEBPS/document_1/document_1.html#_Toc144218049> ;
    dcat:landingPage "https://www.legislation.gov.au/F2021L00313/2023-08-04/2023-08-04/text/original/epub/OEBPS/document_1/document_1.html#_Toc144218049"^^xsd:anyURI ;
    dcat:theme legcons:Division .

F2021L00313:1 a legcons:Chapter,
        owl:Class,
        dcat:Resource ;
    rdfs:label "Chapter - C1 Chapter 1 Preliminary"@en-AU ;
    dct:hasPart F2021L00313:10,
        F2021L00313:11,
        F2021L00313:12,
        F2021L00313:13,
        F2021L00313:14,
        F2021L00313:2,
        F2021L00313:3,
        F2021L00313:4,
        F2021L00313:5,
        F2021L00313:6,
        F2021L00313:7,
        F2021L00313:8,
        F2021L00313:9 ;
    dct:isReferencedBy F2021L00313: ;
    rdfs:comment "Chapter 1 Preliminary - Abrievated Graph Key: C1"@en-AU ;
    skos:broader F2021L00313:10,
        F2021L00313:11,
        F2021L00313:12,
        F2021L00313:13,
        F2021L00313:14,
        F2021L00313:2,
        F2021L00313:3,
        F2021L00313:4,
        F2021L00313:5,
        F2021L00313:6,
        F2021L00313:7,
        F2021L00313:8,
        F2021L00313:9 ;
    skos:definition "Chapter 1 Preliminary"@en-AU ;
    skos:prefLabel "Chapter C1"@en-AU ;
    dcat:accessURL <https://www.legislation.gov.au/F2021L00313/2023-08-04/2023-08-04/text/original/epub/OEBPS/document_1/document_1.html#_Toc144217846> ;
    dcat:landingPage "https://www.legislation.gov.au/F2021L00313/2023-08-04/2023-08-04/text/original/epub/OEBPS/document_1/document_1.html#_Toc144217846"^^xsd:anyURI ;
    dcat:theme legcons:Chapter .

F2021L00313:171 a legcons:Division,
        owl:Class,
        dcat:Resource ;
    rdfs:label "Division - D171 Division 2 General rules relating to official marks"@en-AU ;
    dct:hasPart F2021L00313:172,
        F2021L00313:173,
        F2021L00313:174,
        F2021L00313:175,
        F2021L00313:176,
        F2021L00313:177,
        F2021L00313:178,
        F2021L00313:179,
        F2021L00313:180,
        F2021L00313:181,
        F2021L00313:182,
        F2021L00313:183 ;
    dct:isPartOf F2021L00313:158 ;
    dct:isReferencedBy F2021L00313: ;
    rdfs:comment "Division 2 General rules relating to official marks - Abrievated Graph Key: D171"@en-AU ;
    skos:broader F2021L00313:172,
        F2021L00313:173,
        F2021L00313:174,
        F2021L00313:175,
        F2021L00313:176,
        F2021L00313:177,
        F2021L00313:178,
        F2021L00313:179,
        F2021L00313:180,
        F2021L00313:181,
        F2021L00313:182,
        F2021L00313:183 ;
    skos:definition "Division 2 General rules relating to official marks"@en-AU ;
    skos:narrower F2021L00313:158 ;
    skos:prefLabel "Division D171"@en-AU ;
    dcat:accessURL <https://www.legislation.gov.au/F2021L00313/2023-08-04/2023-08-04/text/original/epub/OEBPS/document_1/document_1.html#_Toc144218016> ;
    dcat:landingPage "https://www.legislation.gov.au/F2021L00313/2023-08-04/2023-08-04/text/original/epub/OEBPS/document_1/document_1.html#_Toc144218016"^^xsd:anyURI ;
    dcat:theme legcons:Division .

F2021L00313:223 a legcons:Division,
        owl:Class,
        dcat:Resource ;
    rdfs:label "Division - D223 Division 2 Functions and powers"@en-AU ;
    dct:hasPart F2021L00313:224,
        F2021L00313:225,
        F2021L00313:226,
        F2021L00313:227,
        F2021L00313:228,
        F2021L00313:229,
        F2021L00313:230,
        F2021L00313:231,
        F2021L00313:232,
        F2021L00313:233,
        F2021L00313:234,
        F2021L00313:235 ;
    dct:isPartOf F2021L00313:220 ;
    dct:isReferencedBy F2021L00313: ;
    rdfs:comment "Division 2 Functions and powers - Abrievated Graph Key: D223"@en-AU ;
    skos:broader F2021L00313:224,
        F2021L00313:225,
        F2021L00313:226,
        F2021L00313:227,
        F2021L00313:228,
        F2021L00313:229,
        F2021L00313:230,
        F2021L00313:231,
        F2021L00313:232,
        F2021L00313:233,
        F2021L00313:234,
        F2021L00313:235 ;
    skos:definition "Division 2 Functions and powers"@en-AU ;
    skos:narrower F2021L00313:220 ;
    skos:prefLabel "Division D223"@en-AU ;
    dcat:accessURL <https://www.legislation.gov.au/F2021L00313/2023-08-04/2023-08-04/text/original/epub/OEBPS/document_1/document_1.html#_Toc144218068> ;
    dcat:landingPage "https://www.legislation.gov.au/F2021L00313/2023-08-04/2023-08-04/text/original/epub/OEBPS/document_1/document_1.html#_Toc144218068"^^xsd:anyURI ;
    dcat:theme legcons:Division .

F2021L00313:267 a legcons:Part,
        owl:Class,
        dcat:Resource ;
    rdfs:label "Part - P267 Part 2 Registered establishments meat inspection services"@en-AU ;
    dct:hasPart F2021L00313:268,
        F2021L00313:269,
        F2021L00313:270,
        F2021L00313:271,
        F2021L00313:272,
        F2021L00313:273,
        F2021L00313:274,
        F2021L00313:275,
        F2021L00313:276,
        F2021L00313:277,
        F2021L00313:278,
        F2021L00313:279,
        F2021L00313:280,
        F2021L00313:281,
        F2021L00313:282,
        F2021L00313:283,
        F2021L00313:284 ;
    dct:isPartOf F2021L00313:264 ;
    dct:isReferencedBy F2021L00313: ;
    rdfs:comment "Part 2 Registered establishments meat inspection services - Abrievated Graph Key: P267"@en-AU ;
    skos:broader F2021L00313:268,
        F2021L00313:269,
        F2021L00313:270,
        F2021L00313:271,
        F2021L00313:272,
        F2021L00313:273,
        F2021L00313:274,
        F2021L00313:275,
        F2021L00313:276,
        F2021L00313:277,
        F2021L00313:278,
        F2021L00313:279,
        F2021L00313:280,
        F2021L00313:281,
        F2021L00313:282,
        F2021L00313:283,
        F2021L00313:284 ;
    skos:definition "Part 2 Registered establishments meat inspection services"@en-AU ;
    skos:narrower F2021L00313:264 ;
    skos:prefLabel "Part P267"@en-AU ;
    dcat:accessURL <https://www.legislation.gov.au/F2021L00313/2023-08-04/2023-08-04/text/original/epub/OEBPS/document_1/document_1.html#_Toc144218112> ;
    dcat:landingPage "https://www.legislation.gov.au/F2021L00313/2023-08-04/2023-08-04/text/original/epub/OEBPS/document_1/document_1.html#_Toc144218112"^^xsd:anyURI ;
    dcat:theme legcons:Part .

F2021L00313: a owl:Class,
        dcat:Dataset,
        dcat:Resource ;
    rdfs:label "Export Control (Wild Game Meat and Wild Game Meat Products) Rules 2021" ;
    dct:Jurisdiction " Department of Agriculture, Fisheries and Forestry "@en-AU ;
    dct:created "2024-08-30T15:14:11.089658"^^xsd:dateTime ;
    dct:creator "https://orcid.org/0009-0007-8434-7325"^^xsd:anyURI ;
    dct:date "2023-08-04T00:00:00+10:00"^^xsd:dateTime ;
    dct:description "Export Control (Wild Game Meat and Wild Game Meat Products) Rules 2021"@en-AU ;
    dct:identifier "https://www.legislation.gov.au/F2021L00313/latest"^^xsd:anyURI ;
    dct:license <https://creativecommons.org/licenses/by-sa/4.0/> ;
    dct:source "scheme=AGLSTERMS.AglsAgent; corporateName=Office Parliamentary Counsel; address=Locked Bag 30 Kingston ACT 2604; contact=+61 2 6120 1400"@en-AU ;
    dct:subject "Export Control (Wild Game Meat and Wild Game Meat Products) Rules 2021"@en-AU ;
    dct:title "Export Control (Wild Game Meat and Wild Game Meat Products) Rules 2021"@en-AU ;
    owl:imports legcons: ;
    dcat:theme legcons:Chapter,
        legcons:Division,
        legcons:Endnotes,
        legcons:Item,
        legcons:Part ;
    schema:identifier "F2021L00313" ;
    schema:status "In force" ;
    schema:version "F2023C00769 (C03)" .

