@prefix F2021L00334: <http://example.org/au/leg/dataset/F2021L00334/> .
@prefix dcat: <http://www.w3.org/ns/dcat#> .
@prefix dct: <http://purl.org/dc/terms/> .
@prefix legcons: <http://example.org/au/leg/concepts/> .
@prefix owl: <http://www.w3.org/2002/07/owl#> .
@prefix rdfs: <http://www.w3.org/2000/01/rdf-schema#> .
@prefix schema: <https://schema.org/> .
@prefix skos: <http://www.w3.org/2004/02/skos/core#> .
@prefix xsd: <http://www.w3.org/2001/XMLSchema#> .

F2021L00334:10 a legcons:Division,
        owl:Class,
        dcat:Resource ;
    rdfs:label "Division - D10 Division 2 Other interpretation provisions"@en-AU ;
    dct:isPartOf F2021L00334:1 ;
    dct:isReferencedBy F2021L00334: ;
    rdfs:comment "Division 2 Other interpretation provisions - Abrievated Graph Key: D10"@en-AU ;
    skos:definition "Division 2 Other interpretation provisions"@en-AU ;
    skos:narrower F2021L00334:1 ;
    skos:prefLabel "Division D10"@en-AU ;
    dcat:accessURL <https://www.legislation.gov.au/F2021L00334/2023-08-04/2023-08-04/text/original/epub/OEBPS/document_1/document_1.html#_Toc143507657> ;
    dcat:landingPage "https://www.legislation.gov.au/F2021L00334/2023-08-04/2023-08-04/text/original/epub/OEBPS/document_1/document_1.html#_Toc143507657"^^xsd:anyURI ;
    dcat:theme legcons:Division .

F2021L00334:100 a legcons:Item,
        owl:Class,
        dcat:Resource ;
    rdfs:label "Item - I100 4 11  Requirements for registration continue to be met"@en-AU ;
    dct:isPartOf F2021L00334:98 ;
    dct:isReferencedBy F2021L00334: ;
    rdfs:comment "4 11  Requirements for registration continue to be met - Abrievated Graph Key: I100"@en-AU ;
    skos:definition "4 11  Requirements for registration continue to be met"@en-AU ;
    skos:narrower F2021L00334:98 ;
    skos:prefLabel "Item I100"@en-AU ;
    dcat:accessURL <https://www.legislation.gov.au/F2021L00334/2023-08-04/2023-08-04/text/original/epub/OEBPS/document_1/document_1.html#_Toc143507747> ;
    dcat:landingPage "https://www.legislation.gov.au/F2021L00334/2023-08-04/2023-08-04/text/original/epub/OEBPS/document_1/document_1.html#_Toc143507747"^^xsd:anyURI ;
    dcat:theme legcons:Item .

F2021L00334:101 a legcons:Item,
        owl:Class,
        dcat:Resource ;
    rdfs:label "Item - I101 4 12  Certificate of registration must be displayed"@en-AU ;
    dct:isPartOf F2021L00334:98 ;
    dct:isReferencedBy F2021L00334: ;
    rdfs:comment "4 12  Certificate of registration must be displayed - Abrievated Graph Key: I101"@en-AU ;
    skos:definition "4 12  Certificate of registration must be displayed"@en-AU ;
    skos:narrower F2021L00334:98 ;
    skos:prefLabel "Item I101"@en-AU ;
    dcat:accessURL <https://www.legislation.gov.au/F2021L00334/2023-08-04/2023-08-04/text/original/epub/OEBPS/document_1/document_1.html#_Toc143507748> ;
    dcat:landingPage "https://www.legislation.gov.au/F2021L00334/2023-08-04/2023-08-04/text/original/epub/OEBPS/document_1/document_1.html#_Toc143507748"^^xsd:anyURI ;
    dcat:theme legcons:Item .

F2021L00334:102 a legcons:Item,
        owl:Class,
        dcat:Resource ;
    rdfs:label "Item - I102 4 13  Notice of certain matters must be given to persons who manage or control export operations at registered establishment"@en-AU ;
    dct:isPartOf F2021L00334:98 ;
    dct:isReferencedBy F2021L00334: ;
    rdfs:comment "4 13  Notice of certain matters must be given to persons who manage or control export operations at registered establishment - Abrievated Graph Key: I102"@en-AU ;
    skos:definition "4 13  Notice of certain matters must be given to persons who manage or control export operations at registered establishment"@en-AU ;
    skos:narrower F2021L00334:98 ;
    skos:prefLabel "Item I102"@en-AU ;
    dcat:accessURL <https://www.legislation.gov.au/F2021L00334/2023-08-04/2023-08-04/text/original/epub/OEBPS/document_1/document_1.html#_Toc143507749> ;
    dcat:landingPage "https://www.legislation.gov.au/F2021L00334/2023-08-04/2023-08-04/text/original/epub/OEBPS/document_1/document_1.html#_Toc143507749"^^xsd:anyURI ;
    dcat:theme legcons:Item .

F2021L00334:103 a legcons:Item,
        owl:Class,
        dcat:Resource ;
    rdfs:label "Item - I103 4 14  List of persons who manage or control export operations at registered establishment"@en-AU ;
    dct:isPartOf F2021L00334:98 ;
    dct:isReferencedBy F2021L00334: ;
    rdfs:comment "4 14  List of persons who manage or control export operations at registered establishment - Abrievated Graph Key: I103"@en-AU ;
    skos:definition "4 14  List of persons who manage or control export operations at registered establishment"@en-AU ;
    skos:narrower F2021L00334:98 ;
    skos:prefLabel "Item I103"@en-AU ;
    dcat:accessURL <https://www.legislation.gov.au/F2021L00334/2023-08-04/2023-08-04/text/original/epub/OEBPS/document_1/document_1.html#_Toc143507750> ;
    dcat:landingPage "https://www.legislation.gov.au/F2021L00334/2023-08-04/2023-08-04/text/original/epub/OEBPS/document_1/document_1.html#_Toc143507750"^^xsd:anyURI ;
    dcat:theme legcons:Item .

F2021L00334:104 a legcons:Item,
        owl:Class,
        dcat:Resource ;
    rdfs:label "Item - I104 4 15  Meat inspection services"@en-AU ;
    dct:isPartOf F2021L00334:98 ;
    dct:isReferencedBy F2021L00334: ;
    rdfs:comment "4 15  Meat inspection services - Abrievated Graph Key: I104"@en-AU ;
    skos:definition "4 15  Meat inspection services"@en-AU ;
    skos:narrower F2021L00334:98 ;
    skos:prefLabel "Item I104"@en-AU ;
    dcat:accessURL <https://www.legislation.gov.au/F2021L00334/2023-08-04/2023-08-04/text/original/epub/OEBPS/document_1/document_1.html#_Toc143507751> ;
    dcat:landingPage "https://www.legislation.gov.au/F2021L00334/2023-08-04/2023-08-04/text/original/epub/OEBPS/document_1/document_1.html#_Toc143507751"^^xsd:anyURI ;
    dcat:theme legcons:Item .

F2021L00334:106 a legcons:Item,
        owl:Class,
        dcat:Resource ;
    rdfs:label "Item - I106 4 16  Period within which application to renew registration must be made"@en-AU ;
    dct:isPartOf F2021L00334:105 ;
    dct:isReferencedBy F2021L00334: ;
    rdfs:comment "4 16  Period within which application to renew registration must be made - Abrievated Graph Key: I106"@en-AU ;
    skos:definition "4 16  Period within which application to renew registration must be made"@en-AU ;
    skos:narrower F2021L00334:105 ;
    skos:prefLabel "Item I106"@en-AU ;
    dcat:accessURL <https://www.legislation.gov.au/F2021L00334/2023-08-04/2023-08-04/text/original/epub/OEBPS/document_1/document_1.html#_Toc143507753> ;
    dcat:landingPage "https://www.legislation.gov.au/F2021L00334/2023-08-04/2023-08-04/text/original/epub/OEBPS/document_1/document_1.html#_Toc143507753"^^xsd:anyURI ;
    dcat:theme legcons:Item .

F2021L00334:107 a legcons:Item,
        owl:Class,
        dcat:Resource ;
    rdfs:label "Item - I107 4 17  Requirements for renewal of registration"@en-AU ;
    dct:isPartOf F2021L00334:105 ;
    dct:isReferencedBy F2021L00334: ;
    rdfs:comment "4 17  Requirements for renewal of registration - Abrievated Graph Key: I107"@en-AU ;
    skos:definition "4 17  Requirements for renewal of registration"@en-AU ;
    skos:narrower F2021L00334:105 ;
    skos:prefLabel "Item I107"@en-AU ;
    dcat:accessURL <https://www.legislation.gov.au/F2021L00334/2023-08-04/2023-08-04/text/original/epub/OEBPS/document_1/document_1.html#_Toc143507754> ;
    dcat:landingPage "https://www.legislation.gov.au/F2021L00334/2023-08-04/2023-08-04/text/original/epub/OEBPS/document_1/document_1.html#_Toc143507754"^^xsd:anyURI ;
    dcat:theme legcons:Item .

F2021L00334:109 a legcons:Item,
        owl:Class,
        dcat:Resource ;
    rdfs:label "Item - I109 4 18  Alterations for which approval is not required"@en-AU ;
    dct:isPartOf F2021L00334:108 ;
    dct:isReferencedBy F2021L00334: ;
    rdfs:comment "4 18  Alterations for which approval is not required - Abrievated Graph Key: I109"@en-AU ;
    skos:definition "4 18  Alterations for which approval is not required"@en-AU ;
    skos:narrower F2021L00334:108 ;
    skos:prefLabel "Item I109"@en-AU ;
    dcat:accessURL <https://www.legislation.gov.au/F2021L00334/2023-08-04/2023-08-04/text/original/epub/OEBPS/document_1/document_1.html#_Toc143507756> ;
    dcat:landingPage "https://www.legislation.gov.au/F2021L00334/2023-08-04/2023-08-04/text/original/epub/OEBPS/document_1/document_1.html#_Toc143507756"^^xsd:anyURI ;
    dcat:theme legcons:Item .

F2021L00334:11 a legcons:Item,
        owl:Class,
        dcat:Resource ;
    rdfs:label "Item - I11 1 7  References to authorised officer and meat safety inspector"@en-AU ;
    dct:isPartOf F2021L00334:1 ;
    dct:isReferencedBy F2021L00334: ;
    rdfs:comment "1 7  References to authorised officer and meat safety inspector - Abrievated Graph Key: I11"@en-AU ;
    skos:definition "1 7  References to authorised officer and meat safety inspector"@en-AU ;
    skos:narrower F2021L00334:1 ;
    skos:prefLabel "Item I11"@en-AU ;
    dcat:accessURL <https://www.legislation.gov.au/F2021L00334/2023-08-04/2023-08-04/text/original/epub/OEBPS/document_1/document_1.html#_Toc143507658> ;
    dcat:landingPage "https://www.legislation.gov.au/F2021L00334/2023-08-04/2023-08-04/text/original/epub/OEBPS/document_1/document_1.html#_Toc143507658"^^xsd:anyURI ;
    dcat:theme legcons:Item .

F2021L00334:111 a legcons:Item,
        owl:Class,
        dcat:Resource ;
    rdfs:label "Item - I111 4 19  Application of this Part"@en-AU ;
    dct:isPartOf F2021L00334:110 ;
    dct:isReferencedBy F2021L00334: ;
    rdfs:comment "4 19  Application of this Part - Abrievated Graph Key: I111"@en-AU ;
    skos:definition "4 19  Application of this Part"@en-AU ;
    skos:narrower F2021L00334:110 ;
    skos:prefLabel "Item I111"@en-AU ;
    dcat:accessURL <https://www.legislation.gov.au/F2021L00334/2023-08-04/2023-08-04/text/original/epub/OEBPS/document_1/document_1.html#_Toc143507758> ;
    dcat:landingPage "https://www.legislation.gov.au/F2021L00334/2023-08-04/2023-08-04/text/original/epub/OEBPS/document_1/document_1.html#_Toc143507758"^^xsd:anyURI ;
    dcat:theme legcons:Item .

F2021L00334:112 a legcons:Item,
        owl:Class,
        dcat:Resource ;
    rdfs:label "Item - I112 4 20  Initial consideration period"@en-AU ;
    dct:isPartOf F2021L00334:110 ;
    dct:isReferencedBy F2021L00334: ;
    rdfs:comment "4 20  Initial consideration period - Abrievated Graph Key: I112"@en-AU ;
    skos:definition "4 20  Initial consideration period"@en-AU ;
    skos:narrower F2021L00334:110 ;
    skos:prefLabel "Item I112"@en-AU ;
    dcat:accessURL <https://www.legislation.gov.au/F2021L00334/2023-08-04/2023-08-04/text/original/epub/OEBPS/document_1/document_1.html#_Toc143507759> ;
    dcat:landingPage "https://www.legislation.gov.au/F2021L00334/2023-08-04/2023-08-04/text/original/epub/OEBPS/document_1/document_1.html#_Toc143507759"^^xsd:anyURI ;
    dcat:theme legcons:Item .

F2021L00334:113 a legcons:Item,
        owl:Class,
        dcat:Resource ;
    rdfs:label "Item - I113 4 21  Period within which request relating to application must be complied with"@en-AU ;
    dct:isPartOf F2021L00334:110 ;
    dct:isReferencedBy F2021L00334: ;
    rdfs:comment "4 21  Period within which request relating to application must be complied with - Abrievated Graph Key: I113"@en-AU ;
    skos:definition "4 21  Period within which request relating to application must be complied with"@en-AU ;
    skos:narrower F2021L00334:110 ;
    skos:prefLabel "Item I113"@en-AU ;
    dcat:accessURL <https://www.legislation.gov.au/F2021L00334/2023-08-04/2023-08-04/text/original/epub/OEBPS/document_1/document_1.html#_Toc143507760> ;
    dcat:landingPage "https://www.legislation.gov.au/F2021L00334/2023-08-04/2023-08-04/text/original/epub/OEBPS/document_1/document_1.html#_Toc143507760"^^xsd:anyURI ;
    dcat:theme legcons:Item .

F2021L00334:116 a legcons:Item,
        owl:Class,
        dcat:Resource ;
    rdfs:label "Item - I116 4 22  Application for allocation of meat inspection services to establishment"@en-AU ;
    dct:isPartOf F2021L00334:115 ;
    dct:isReferencedBy F2021L00334: ;
    rdfs:comment "4 22  Application for allocation of meat inspection services to establishment - Abrievated Graph Key: I116"@en-AU ;
    skos:definition "4 22  Application for allocation of meat inspection services to establishment"@en-AU ;
    skos:narrower F2021L00334:115 ;
    skos:prefLabel "Item I116"@en-AU ;
    dcat:accessURL <https://www.legislation.gov.au/F2021L00334/2023-08-04/2023-08-04/text/original/epub/OEBPS/document_1/document_1.html#_Toc143507763> ;
    dcat:landingPage "https://www.legislation.gov.au/F2021L00334/2023-08-04/2023-08-04/text/original/epub/OEBPS/document_1/document_1.html#_Toc143507763"^^xsd:anyURI ;
    dcat:theme legcons:Item .

F2021L00334:117 a legcons:Item,
        owl:Class,
        dcat:Resource ;
    rdfs:label "Item - I117 4 23  Preliminary allocation"@en-AU ;
    dct:isPartOf F2021L00334:115 ;
    dct:isReferencedBy F2021L00334: ;
    rdfs:comment "4 23  Preliminary allocation - Abrievated Graph Key: I117"@en-AU ;
    skos:definition "4 23  Preliminary allocation"@en-AU ;
    skos:narrower F2021L00334:115 ;
    skos:prefLabel "Item I117"@en-AU ;
    dcat:accessURL <https://www.legislation.gov.au/F2021L00334/2023-08-04/2023-08-04/text/original/epub/OEBPS/document_1/document_1.html#_Toc143507764> ;
    dcat:landingPage "https://www.legislation.gov.au/F2021L00334/2023-08-04/2023-08-04/text/original/epub/OEBPS/document_1/document_1.html#_Toc143507764"^^xsd:anyURI ;
    dcat:theme legcons:Item .

F2021L00334:118 a legcons:Item,
        owl:Class,
        dcat:Resource ;
    rdfs:label "Item - I118 4 24  Notice of preliminary allocation"@en-AU ;
    dct:isPartOf F2021L00334:115 ;
    dct:isReferencedBy F2021L00334: ;
    rdfs:comment "4 24  Notice of preliminary allocation - Abrievated Graph Key: I118"@en-AU ;
    skos:definition "4 24  Notice of preliminary allocation"@en-AU ;
    skos:narrower F2021L00334:115 ;
    skos:prefLabel "Item I118"@en-AU ;
    dcat:accessURL <https://www.legislation.gov.au/F2021L00334/2023-08-04/2023-08-04/text/original/epub/OEBPS/document_1/document_1.html#_Toc143507765> ;
    dcat:landingPage "https://www.legislation.gov.au/F2021L00334/2023-08-04/2023-08-04/text/original/epub/OEBPS/document_1/document_1.html#_Toc143507765"^^xsd:anyURI ;
    dcat:theme legcons:Item .

F2021L00334:119 a legcons:Item,
        owl:Class,
        dcat:Resource ;
    rdfs:label "Item - I119 4 25  Procedure following notice of preliminary allocation"@en-AU ;
    dct:isPartOf F2021L00334:115 ;
    dct:isReferencedBy F2021L00334: ;
    rdfs:comment "4 25  Procedure following notice of preliminary allocation - Abrievated Graph Key: I119"@en-AU ;
    skos:definition "4 25  Procedure following notice of preliminary allocation"@en-AU ;
    skos:narrower F2021L00334:115 ;
    skos:prefLabel "Item I119"@en-AU ;
    dcat:accessURL <https://www.legislation.gov.au/F2021L00334/2023-08-04/2023-08-04/text/original/epub/OEBPS/document_1/document_1.html#_Toc143507766> ;
    dcat:landingPage "https://www.legislation.gov.au/F2021L00334/2023-08-04/2023-08-04/text/original/epub/OEBPS/document_1/document_1.html#_Toc143507766"^^xsd:anyURI ;
    dcat:theme legcons:Item .

F2021L00334:12 a legcons:Item,
        owl:Class,
        dcat:Resource ;
    rdfs:label "Item - I12 1 8  Modifications of certain terms used in the Australian Meat Standard"@en-AU ;
    dct:isPartOf F2021L00334:1 ;
    dct:isReferencedBy F2021L00334: ;
    rdfs:comment "1 8  Modifications of certain terms used in the Australian Meat Standard - Abrievated Graph Key: I12"@en-AU ;
    skos:definition "1 8  Modifications of certain terms used in the Australian Meat Standard"@en-AU ;
    skos:narrower F2021L00334:1 ;
    skos:prefLabel "Item I12"@en-AU ;
    dcat:accessURL <https://www.legislation.gov.au/F2021L00334/2023-08-04/2023-08-04/text/original/epub/OEBPS/document_1/document_1.html#_Toc143507659> ;
    dcat:landingPage "https://www.legislation.gov.au/F2021L00334/2023-08-04/2023-08-04/text/original/epub/OEBPS/document_1/document_1.html#_Toc143507659"^^xsd:anyURI ;
    dcat:theme legcons:Item .

F2021L00334:120 a legcons:Item,
        owl:Class,
        dcat:Resource ;
    rdfs:label "Item - I120 4 26  Revised allocation"@en-AU ;
    dct:isPartOf F2021L00334:115 ;
    dct:isReferencedBy F2021L00334: ;
    rdfs:comment "4 26  Revised allocation - Abrievated Graph Key: I120"@en-AU ;
    skos:definition "4 26  Revised allocation"@en-AU ;
    skos:narrower F2021L00334:115 ;
    skos:prefLabel "Item I120"@en-AU ;
    dcat:accessURL <https://www.legislation.gov.au/F2021L00334/2023-08-04/2023-08-04/text/original/epub/OEBPS/document_1/document_1.html#_Toc143507767> ;
    dcat:landingPage "https://www.legislation.gov.au/F2021L00334/2023-08-04/2023-08-04/text/original/epub/OEBPS/document_1/document_1.html#_Toc143507767"^^xsd:anyURI ;
    dcat:theme legcons:Item .

F2021L00334:121 a legcons:Item,
        owl:Class,
        dcat:Resource ;
    rdfs:label "Item - I121 4 27  Procedure following notice of revised allocation"@en-AU ;
    dct:isPartOf F2021L00334:115 ;
    dct:isReferencedBy F2021L00334: ;
    rdfs:comment "4 27  Procedure following notice of revised allocation - Abrievated Graph Key: I121"@en-AU ;
    skos:definition "4 27  Procedure following notice of revised allocation"@en-AU ;
    skos:narrower F2021L00334:115 ;
    skos:prefLabel "Item I121"@en-AU ;
    dcat:accessURL <https://www.legislation.gov.au/F2021L00334/2023-08-04/2023-08-04/text/original/epub/OEBPS/document_1/document_1.html#_Toc143507768> ;
    dcat:landingPage "https://www.legislation.gov.au/F2021L00334/2023-08-04/2023-08-04/text/original/epub/OEBPS/document_1/document_1.html#_Toc143507768"^^xsd:anyURI ;
    dcat:theme legcons:Item .

F2021L00334:122 a legcons:Item,
        owl:Class,
        dcat:Resource ;
    rdfs:label "Item - I122 4 28  Review of Secretarys determination"@en-AU ;
    dct:isPartOf F2021L00334:115 ;
    dct:isReferencedBy F2021L00334: ;
    rdfs:comment "4 28  Review of Secretarys determination - Abrievated Graph Key: I122"@en-AU ;
    skos:definition "4 28  Review of Secretarys determination"@en-AU ;
    skos:narrower F2021L00334:115 ;
    skos:prefLabel "Item I122"@en-AU ;
    dcat:accessURL <https://www.legislation.gov.au/F2021L00334/2023-08-04/2023-08-04/text/original/epub/OEBPS/document_1/document_1.html#_Toc143507769> ;
    dcat:landingPage "https://www.legislation.gov.au/F2021L00334/2023-08-04/2023-08-04/text/original/epub/OEBPS/document_1/document_1.html#_Toc143507769"^^xsd:anyURI ;
    dcat:theme legcons:Item .

F2021L00334:123 a legcons:Item,
        owl:Class,
        dcat:Resource ;
    rdfs:label "Item - I123 4 29  Determination of new allocation"@en-AU ;
    dct:isPartOf F2021L00334:115 ;
    dct:isReferencedBy F2021L00334: ;
    rdfs:comment "4 29  Determination of new allocation - Abrievated Graph Key: I123"@en-AU ;
    skos:definition "4 29  Determination of new allocation"@en-AU ;
    skos:narrower F2021L00334:115 ;
    skos:prefLabel "Item I123"@en-AU ;
    dcat:accessURL <https://www.legislation.gov.au/F2021L00334/2023-08-04/2023-08-04/text/original/epub/OEBPS/document_1/document_1.html#_Toc143507770> ;
    dcat:landingPage "https://www.legislation.gov.au/F2021L00334/2023-08-04/2023-08-04/text/original/epub/OEBPS/document_1/document_1.html#_Toc143507770"^^xsd:anyURI ;
    dcat:theme legcons:Item .

F2021L00334:125 a legcons:Item,
        owl:Class,
        dcat:Resource ;
    rdfs:label "Item - I125 4 30  Application to vary allocation of meat inspection services"@en-AU ;
    dct:isPartOf F2021L00334:124 ;
    dct:isReferencedBy F2021L00334: ;
    rdfs:comment "4 30  Application to vary allocation of meat inspection services - Abrievated Graph Key: I125"@en-AU ;
    skos:definition "4 30  Application to vary allocation of meat inspection services"@en-AU ;
    skos:narrower F2021L00334:124 ;
    skos:prefLabel "Item I125"@en-AU ;
    dcat:accessURL <https://www.legislation.gov.au/F2021L00334/2023-08-04/2023-08-04/text/original/epub/OEBPS/document_1/document_1.html#_Toc143507772> ;
    dcat:landingPage "https://www.legislation.gov.au/F2021L00334/2023-08-04/2023-08-04/text/original/epub/OEBPS/document_1/document_1.html#_Toc143507772"^^xsd:anyURI ;
    dcat:theme legcons:Item .

F2021L00334:126 a legcons:Item,
        owl:Class,
        dcat:Resource ;
    rdfs:label "Item - I126 4 31  Application for additional allocation of meat inspection services"@en-AU ;
    dct:isPartOf F2021L00334:124 ;
    dct:isReferencedBy F2021L00334: ;
    rdfs:comment "4 31  Application for additional allocation of meat inspection services - Abrievated Graph Key: I126"@en-AU ;
    skos:definition "4 31  Application for additional allocation of meat inspection services"@en-AU ;
    skos:narrower F2021L00334:124 ;
    skos:prefLabel "Item I126"@en-AU ;
    dcat:accessURL <https://www.legislation.gov.au/F2021L00334/2023-08-04/2023-08-04/text/original/epub/OEBPS/document_1/document_1.html#_Toc143507773> ;
    dcat:landingPage "https://www.legislation.gov.au/F2021L00334/2023-08-04/2023-08-04/text/original/epub/OEBPS/document_1/document_1.html#_Toc143507773"^^xsd:anyURI ;
    dcat:theme legcons:Item .

F2021L00334:127 a legcons:Item,
        owl:Class,
        dcat:Resource ;
    rdfs:label "Item - I127 4 32  Notification that meat inspection services not required during shutdown period"@en-AU ;
    dct:isPartOf F2021L00334:124 ;
    dct:isReferencedBy F2021L00334: ;
    rdfs:comment "4 32  Notification that meat inspection services not required during shutdown period - Abrievated Graph Key: I127"@en-AU ;
    skos:definition "4 32  Notification that meat inspection services not required during shutdown period"@en-AU ;
    skos:narrower F2021L00334:124 ;
    skos:prefLabel "Item I127"@en-AU ;
    dcat:accessURL <https://www.legislation.gov.au/F2021L00334/2023-08-04/2023-08-04/text/original/epub/OEBPS/document_1/document_1.html#_Toc143507774> ;
    dcat:landingPage "https://www.legislation.gov.au/F2021L00334/2023-08-04/2023-08-04/text/original/epub/OEBPS/document_1/document_1.html#_Toc143507774"^^xsd:anyURI ;
    dcat:theme legcons:Item .

F2021L00334:128 a legcons:Item,
        owl:Class,
        dcat:Resource ;
    rdfs:label "Item - I128 4 33  Variation by Secretary of allocation of meat inspection services"@en-AU ;
    dct:isPartOf F2021L00334:124 ;
    dct:isReferencedBy F2021L00334: ;
    rdfs:comment "4 33  Variation by Secretary of allocation of meat inspection services - Abrievated Graph Key: I128"@en-AU ;
    skos:definition "4 33  Variation by Secretary of allocation of meat inspection services"@en-AU ;
    skos:narrower F2021L00334:124 ;
    skos:prefLabel "Item I128"@en-AU ;
    dcat:accessURL <https://www.legislation.gov.au/F2021L00334/2023-08-04/2023-08-04/text/original/epub/OEBPS/document_1/document_1.html#_Toc143507775> ;
    dcat:landingPage "https://www.legislation.gov.au/F2021L00334/2023-08-04/2023-08-04/text/original/epub/OEBPS/document_1/document_1.html#_Toc143507775"^^xsd:anyURI ;
    dcat:theme legcons:Item .

F2021L00334:129 a legcons:Item,
        owl:Class,
        dcat:Resource ;
    rdfs:label "Item - I129 4 34  Notification of termination of meat inspection services"@en-AU ;
    dct:isPartOf F2021L00334:124 ;
    dct:isReferencedBy F2021L00334: ;
    rdfs:comment "4 34  Notification of termination of meat inspection services - Abrievated Graph Key: I129"@en-AU ;
    skos:definition "4 34  Notification of termination of meat inspection services"@en-AU ;
    skos:narrower F2021L00334:124 ;
    skos:prefLabel "Item I129"@en-AU ;
    dcat:accessURL <https://www.legislation.gov.au/F2021L00334/2023-08-04/2023-08-04/text/original/epub/OEBPS/document_1/document_1.html#_Toc143507776> ;
    dcat:landingPage "https://www.legislation.gov.au/F2021L00334/2023-08-04/2023-08-04/text/original/epub/OEBPS/document_1/document_1.html#_Toc143507776"^^xsd:anyURI ;
    dcat:theme legcons:Item .

F2021L00334:13 a legcons:Item,
        owl:Class,
        dcat:Resource ;
    rdfs:label "Item - I13 1 9  Circumstances in which alternative procedure standard or other requirement is taken to meet requirements of Australian Meat Standard"@en-AU ;
    dct:isPartOf F2021L00334:1 ;
    dct:isReferencedBy F2021L00334: ;
    rdfs:comment "1 9  Circumstances in which alternative procedure standard or other requirement is taken to meet requirements of Australian Meat Standard - Abrievated Graph Key: I13"@en-AU ;
    skos:definition "1 9  Circumstances in which alternative procedure standard or other requirement is taken to meet requirements of Australian Meat Standard"@en-AU ;
    skos:narrower F2021L00334:1 ;
    skos:prefLabel "Item I13"@en-AU ;
    dcat:accessURL <https://www.legislation.gov.au/F2021L00334/2023-08-04/2023-08-04/text/original/epub/OEBPS/document_1/document_1.html#_Toc143507660> ;
    dcat:landingPage "https://www.legislation.gov.au/F2021L00334/2023-08-04/2023-08-04/text/original/epub/OEBPS/document_1/document_1.html#_Toc143507660"^^xsd:anyURI ;
    dcat:theme legcons:Item .

F2021L00334:133 a legcons:Item,
        owl:Class,
        dcat:Resource ;
    rdfs:label "Item - I133 5 1  Purpose of this Division"@en-AU ;
    dct:isPartOf F2021L00334:132 ;
    dct:isReferencedBy F2021L00334: ;
    rdfs:comment "5 1  Purpose of this Division - Abrievated Graph Key: I133"@en-AU ;
    skos:definition "5 1  Purpose of this Division"@en-AU ;
    skos:narrower F2021L00334:132 ;
    skos:prefLabel "Item I133"@en-AU ;
    dcat:accessURL <https://www.legislation.gov.au/F2021L00334/2023-08-04/2023-08-04/text/original/epub/OEBPS/document_1/document_1.html#_Toc143507780> ;
    dcat:landingPage "https://www.legislation.gov.au/F2021L00334/2023-08-04/2023-08-04/text/original/epub/OEBPS/document_1/document_1.html#_Toc143507780"^^xsd:anyURI ;
    dcat:theme legcons:Item .

F2021L00334:134 a legcons:Item,
        owl:Class,
        dcat:Resource ;
    rdfs:label "Item - I134 5 2  Other requirementsproposed arrangement for operations to prepare prescribed meat or meat products"@en-AU ;
    dct:isPartOf F2021L00334:132 ;
    dct:isReferencedBy F2021L00334: ;
    rdfs:comment "5 2  Other requirementsproposed arrangement for operations to prepare prescribed meat or meat products - Abrievated Graph Key: I134"@en-AU ;
    skos:definition "5 2  Other requirementsproposed arrangement for operations to prepare prescribed meat or meat products"@en-AU ;
    skos:narrower F2021L00334:132 ;
    skos:prefLabel "Item I134"@en-AU ;
    dcat:accessURL <https://www.legislation.gov.au/F2021L00334/2023-08-04/2023-08-04/text/original/epub/OEBPS/document_1/document_1.html#_Toc143507781> ;
    dcat:landingPage "https://www.legislation.gov.au/F2021L00334/2023-08-04/2023-08-04/text/original/epub/OEBPS/document_1/document_1.html#_Toc143507781"^^xsd:anyURI ;
    dcat:theme legcons:Item .

F2021L00334:135 a legcons:Item,
        owl:Class,
        dcat:Resource ;
    rdfs:label "Item - I135 5 3  Other requirementsproposed arrangement for operations to prepare Halal meat"@en-AU ;
    dct:isPartOf F2021L00334:132 ;
    dct:isReferencedBy F2021L00334: ;
    rdfs:comment "5 3  Other requirementsproposed arrangement for operations to prepare Halal meat - Abrievated Graph Key: I135"@en-AU ;
    skos:definition "5 3  Other requirementsproposed arrangement for operations to prepare Halal meat"@en-AU ;
    skos:narrower F2021L00334:132 ;
    skos:prefLabel "Item I135"@en-AU ;
    dcat:accessURL <https://www.legislation.gov.au/F2021L00334/2023-08-04/2023-08-04/text/original/epub/OEBPS/document_1/document_1.html#_Toc143507782> ;
    dcat:landingPage "https://www.legislation.gov.au/F2021L00334/2023-08-04/2023-08-04/text/original/epub/OEBPS/document_1/document_1.html#_Toc143507782"^^xsd:anyURI ;
    dcat:theme legcons:Item .

F2021L00334:138 a legcons:Item,
        owl:Class,
        dcat:Resource ;
    rdfs:label "Item - I138 5 4  Purpose of this Division"@en-AU ;
    dct:isPartOf F2021L00334:137 ;
    dct:isReferencedBy F2021L00334: ;
    rdfs:comment "5 4  Purpose of this Division - Abrievated Graph Key: I138"@en-AU ;
    skos:definition "5 4  Purpose of this Division"@en-AU ;
    skos:narrower F2021L00334:137 ;
    skos:prefLabel "Item I138"@en-AU ;
    dcat:accessURL <https://www.legislation.gov.au/F2021L00334/2023-08-04/2023-08-04/text/original/epub/OEBPS/document_1/document_1.html#_Toc143507785> ;
    dcat:landingPage "https://www.legislation.gov.au/F2021L00334/2023-08-04/2023-08-04/text/original/epub/OEBPS/document_1/document_1.html#_Toc143507785"^^xsd:anyURI ;
    dcat:theme legcons:Item .

F2021L00334:139 a legcons:Subdivision,
        owl:Class,
        dcat:Resource ;
    rdfs:label "Subdivision - S139 Subdivision BGeneral"@en-AU ;
    dct:isPartOf F2021L00334:136 ;
    dct:isReferencedBy F2021L00334: ;
    rdfs:comment "Subdivision BGeneral - Abrievated Graph Key: S139"@en-AU ;
    skos:definition "Subdivision BGeneral"@en-AU ;
    skos:narrower F2021L00334:136 ;
    skos:prefLabel "Subdivision S139"@en-AU ;
    dcat:accessURL <https://www.legislation.gov.au/F2021L00334/2023-08-04/2023-08-04/text/original/epub/OEBPS/document_1/document_1.html#_Toc143507786> ;
    dcat:landingPage "https://www.legislation.gov.au/F2021L00334/2023-08-04/2023-08-04/text/original/epub/OEBPS/document_1/document_1.html#_Toc143507786"^^xsd:anyURI ;
    dcat:theme legcons:Subdivision .

F2021L00334:140 a legcons:Item,
        owl:Class,
        dcat:Resource ;
    rdfs:label "Item - I140 5 5  Importing country requirements must be met"@en-AU ;
    dct:isPartOf F2021L00334:136 ;
    dct:isReferencedBy F2021L00334: ;
    rdfs:comment "5 5  Importing country requirements must be met - Abrievated Graph Key: I140"@en-AU ;
    skos:definition "5 5  Importing country requirements must be met"@en-AU ;
    skos:narrower F2021L00334:136 ;
    skos:prefLabel "Item I140"@en-AU ;
    dcat:accessURL <https://www.legislation.gov.au/F2021L00334/2023-08-04/2023-08-04/text/original/epub/OEBPS/document_1/document_1.html#_Toc143507787> ;
    dcat:landingPage "https://www.legislation.gov.au/F2021L00334/2023-08-04/2023-08-04/text/original/epub/OEBPS/document_1/document_1.html#_Toc143507787"^^xsd:anyURI ;
    dcat:theme legcons:Item .

F2021L00334:141 a legcons:Item,
        owl:Class,
        dcat:Resource ;
    rdfs:label "Item - I141 5 6  Requirements of Australian Meat Standard must be met"@en-AU ;
    dct:isPartOf F2021L00334:136 ;
    dct:isReferencedBy F2021L00334: ;
    rdfs:comment "5 6  Requirements of Australian Meat Standard must be met - Abrievated Graph Key: I141"@en-AU ;
    skos:definition "5 6  Requirements of Australian Meat Standard must be met"@en-AU ;
    skos:narrower F2021L00334:136 ;
    skos:prefLabel "Item I141"@en-AU ;
    dcat:accessURL <https://www.legislation.gov.au/F2021L00334/2023-08-04/2023-08-04/text/original/epub/OEBPS/document_1/document_1.html#_Toc143507788> ;
    dcat:landingPage "https://www.legislation.gov.au/F2021L00334/2023-08-04/2023-08-04/text/original/epub/OEBPS/document_1/document_1.html#_Toc143507788"^^xsd:anyURI ;
    dcat:theme legcons:Item .

F2021L00334:142 a legcons:Subdivision,
        owl:Class,
        dcat:Resource ;
    rdfs:label "Subdivision - S142 Subdivision CPreparation and transport"@en-AU ;
    dct:isPartOf F2021L00334:136 ;
    dct:isReferencedBy F2021L00334: ;
    rdfs:comment "Subdivision CPreparation and transport - Abrievated Graph Key: S142"@en-AU ;
    skos:definition "Subdivision CPreparation and transport"@en-AU ;
    skos:narrower F2021L00334:136 ;
    skos:prefLabel "Subdivision S142"@en-AU ;
    dcat:accessURL <https://www.legislation.gov.au/F2021L00334/2023-08-04/2023-08-04/text/original/epub/OEBPS/document_1/document_1.html#_Toc143507789> ;
    dcat:landingPage "https://www.legislation.gov.au/F2021L00334/2023-08-04/2023-08-04/text/original/epub/OEBPS/document_1/document_1.html#_Toc143507789"^^xsd:anyURI ;
    dcat:theme legcons:Subdivision .

F2021L00334:143 a legcons:Item,
        owl:Class,
        dcat:Resource ;
    rdfs:label "Item - I143 5 7  Dressing an animal"@en-AU ;
    dct:isPartOf F2021L00334:136 ;
    dct:isReferencedBy F2021L00334: ;
    rdfs:comment "5 7  Dressing an animal - Abrievated Graph Key: I143"@en-AU ;
    skos:definition "5 7  Dressing an animal"@en-AU ;
    skos:narrower F2021L00334:136 ;
    skos:prefLabel "Item I143"@en-AU ;
    dcat:accessURL <https://www.legislation.gov.au/F2021L00334/2023-08-04/2023-08-04/text/original/epub/OEBPS/document_1/document_1.html#_Toc143507790> ;
    dcat:landingPage "https://www.legislation.gov.au/F2021L00334/2023-08-04/2023-08-04/text/original/epub/OEBPS/document_1/document_1.html#_Toc143507790"^^xsd:anyURI ;
    dcat:theme legcons:Item .

F2021L00334:144 a legcons:Item,
        owl:Class,
        dcat:Resource ;
    rdfs:label "Item - I144 5 8  Areas where post mortem inspections are carried out"@en-AU ;
    dct:isPartOf F2021L00334:136 ;
    dct:isReferencedBy F2021L00334: ;
    rdfs:comment "5 8  Areas where post mortem inspections are carried out - Abrievated Graph Key: I144"@en-AU ;
    skos:definition "5 8  Areas where post mortem inspections are carried out"@en-AU ;
    skos:narrower F2021L00334:136 ;
    skos:prefLabel "Item I144"@en-AU ;
    dcat:accessURL <https://www.legislation.gov.au/F2021L00334/2023-08-04/2023-08-04/text/original/epub/OEBPS/document_1/document_1.html#_Toc143507791> ;
    dcat:landingPage "https://www.legislation.gov.au/F2021L00334/2023-08-04/2023-08-04/text/original/epub/OEBPS/document_1/document_1.html#_Toc143507791"^^xsd:anyURI ;
    dcat:theme legcons:Item .

F2021L00334:145 a legcons:Item,
        owl:Class,
        dcat:Resource ;
    rdfs:label "Item - I145 5 9  Compliance with decisions and dispositions"@en-AU ;
    dct:isPartOf F2021L00334:136 ;
    dct:isReferencedBy F2021L00334: ;
    rdfs:comment "5 9  Compliance with decisions and dispositions - Abrievated Graph Key: I145"@en-AU ;
    skos:definition "5 9  Compliance with decisions and dispositions"@en-AU ;
    skos:narrower F2021L00334:136 ;
    skos:prefLabel "Item I145"@en-AU ;
    dcat:accessURL <https://www.legislation.gov.au/F2021L00334/2023-08-04/2023-08-04/text/original/epub/OEBPS/document_1/document_1.html#_Toc143507792> ;
    dcat:landingPage "https://www.legislation.gov.au/F2021L00334/2023-08-04/2023-08-04/text/original/epub/OEBPS/document_1/document_1.html#_Toc143507792"^^xsd:anyURI ;
    dcat:theme legcons:Item .

F2021L00334:146 a legcons:Item,
        owl:Class,
        dcat:Resource ;
    rdfs:label "Item - I146 5 10  Chilling carcases and carcase parts"@en-AU ;
    dct:isPartOf F2021L00334:136 ;
    dct:isReferencedBy F2021L00334: ;
    rdfs:comment "5 10  Chilling carcases and carcase parts - Abrievated Graph Key: I146"@en-AU ;
    skos:definition "5 10  Chilling carcases and carcase parts"@en-AU ;
    skos:narrower F2021L00334:136 ;
    skos:prefLabel "Item I146"@en-AU ;
    dcat:accessURL <https://www.legislation.gov.au/F2021L00334/2023-08-04/2023-08-04/text/original/epub/OEBPS/document_1/document_1.html#_Toc143507793> ;
    dcat:landingPage "https://www.legislation.gov.au/F2021L00334/2023-08-04/2023-08-04/text/original/epub/OEBPS/document_1/document_1.html#_Toc143507793"^^xsd:anyURI ;
    dcat:theme legcons:Item .

F2021L00334:147 a legcons:Item,
        owl:Class,
        dcat:Resource ;
    rdfs:label "Item - I147 5 11  Temperature controls for and after processing raw meat"@en-AU ;
    dct:isPartOf F2021L00334:136 ;
    dct:isReferencedBy F2021L00334: ;
    rdfs:comment "5 11  Temperature controls for and after processing raw meat - Abrievated Graph Key: I147"@en-AU ;
    skos:definition "5 11  Temperature controls for and after processing raw meat"@en-AU ;
    skos:narrower F2021L00334:136 ;
    skos:prefLabel "Item I147"@en-AU ;
    dcat:accessURL <https://www.legislation.gov.au/F2021L00334/2023-08-04/2023-08-04/text/original/epub/OEBPS/document_1/document_1.html#_Toc143507794> ;
    dcat:landingPage "https://www.legislation.gov.au/F2021L00334/2023-08-04/2023-08-04/text/original/epub/OEBPS/document_1/document_1.html#_Toc143507794"^^xsd:anyURI ;
    dcat:theme legcons:Item .

F2021L00334:148 a legcons:Item,
        owl:Class,
        dcat:Resource ;
    rdfs:label "Item - I148 5 12  Temperature requirements for storing handling and transporting certain prescribed meat or meat products"@en-AU ;
    dct:isPartOf F2021L00334:136 ;
    dct:isReferencedBy F2021L00334: ;
    rdfs:comment "5 12  Temperature requirements for storing handling and transporting certain prescribed meat or meat products - Abrievated Graph Key: I148"@en-AU ;
    skos:definition "5 12  Temperature requirements for storing handling and transporting certain prescribed meat or meat products"@en-AU ;
    skos:narrower F2021L00334:136 ;
    skos:prefLabel "Item I148"@en-AU ;
    dcat:accessURL <https://www.legislation.gov.au/F2021L00334/2023-08-04/2023-08-04/text/original/epub/OEBPS/document_1/document_1.html#_Toc143507795> ;
    dcat:landingPage "https://www.legislation.gov.au/F2021L00334/2023-08-04/2023-08-04/text/original/epub/OEBPS/document_1/document_1.html#_Toc143507795"^^xsd:anyURI ;
    dcat:theme legcons:Item .

F2021L00334:149 a legcons:Item,
        owl:Class,
        dcat:Resource ;
    rdfs:label "Item - I149 5 13  Assessing the effectiveness of refrigeration"@en-AU ;
    dct:isPartOf F2021L00334:136 ;
    dct:isReferencedBy F2021L00334: ;
    rdfs:comment "5 13  Assessing the effectiveness of refrigeration - Abrievated Graph Key: I149"@en-AU ;
    skos:definition "5 13  Assessing the effectiveness of refrigeration"@en-AU ;
    skos:narrower F2021L00334:136 ;
    skos:prefLabel "Item I149"@en-AU ;
    dcat:accessURL <https://www.legislation.gov.au/F2021L00334/2023-08-04/2023-08-04/text/original/epub/OEBPS/document_1/document_1.html#_Toc143507796> ;
    dcat:landingPage "https://www.legislation.gov.au/F2021L00334/2023-08-04/2023-08-04/text/original/epub/OEBPS/document_1/document_1.html#_Toc143507796"^^xsd:anyURI ;
    dcat:theme legcons:Item .

F2021L00334:150 a legcons:Item,
        owl:Class,
        dcat:Resource ;
    rdfs:label "Item - I150 5 14  Thawing of meat"@en-AU ;
    dct:isPartOf F2021L00334:136 ;
    dct:isReferencedBy F2021L00334: ;
    rdfs:comment "5 14  Thawing of meat - Abrievated Graph Key: I150"@en-AU ;
    skos:definition "5 14  Thawing of meat"@en-AU ;
    skos:narrower F2021L00334:136 ;
    skos:prefLabel "Item I150"@en-AU ;
    dcat:accessURL <https://www.legislation.gov.au/F2021L00334/2023-08-04/2023-08-04/text/original/epub/OEBPS/document_1/document_1.html#_Toc143507797> ;
    dcat:landingPage "https://www.legislation.gov.au/F2021L00334/2023-08-04/2023-08-04/text/original/epub/OEBPS/document_1/document_1.html#_Toc143507797"^^xsd:anyURI ;
    dcat:theme legcons:Item .

F2021L00334:151 a legcons:Item,
        owl:Class,
        dcat:Resource ;
    rdfs:label "Item - I151 5 15  Loading prescribed meat or meat products for transfer between registered establishments"@en-AU ;
    dct:isPartOf F2021L00334:136 ;
    dct:isReferencedBy F2021L00334: ;
    rdfs:comment "5 15  Loading prescribed meat or meat products for transfer between registered establishments - Abrievated Graph Key: I151"@en-AU ;
    skos:definition "5 15  Loading prescribed meat or meat products for transfer between registered establishments"@en-AU ;
    skos:narrower F2021L00334:136 ;
    skos:prefLabel "Item I151"@en-AU ;
    dcat:accessURL <https://www.legislation.gov.au/F2021L00334/2023-08-04/2023-08-04/text/original/epub/OEBPS/document_1/document_1.html#_Toc143507798> ;
    dcat:landingPage "https://www.legislation.gov.au/F2021L00334/2023-08-04/2023-08-04/text/original/epub/OEBPS/document_1/document_1.html#_Toc143507798"^^xsd:anyURI ;
    dcat:theme legcons:Item .

F2021L00334:152 a legcons:Item,
        owl:Class,
        dcat:Resource ;
    rdfs:label "Item - I152 5 16  Loading of prescribed meat or meat productssupervision"@en-AU ;
    dct:isPartOf F2021L00334:136 ;
    dct:isReferencedBy F2021L00334: ;
    rdfs:comment "5 16  Loading of prescribed meat or meat productssupervision - Abrievated Graph Key: I152"@en-AU ;
    skos:definition "5 16  Loading of prescribed meat or meat productssupervision"@en-AU ;
    skos:narrower F2021L00334:136 ;
    skos:prefLabel "Item I152"@en-AU ;
    dcat:accessURL <https://www.legislation.gov.au/F2021L00334/2023-08-04/2023-08-04/text/original/epub/OEBPS/document_1/document_1.html#_Toc143507799> ;
    dcat:landingPage "https://www.legislation.gov.au/F2021L00334/2023-08-04/2023-08-04/text/original/epub/OEBPS/document_1/document_1.html#_Toc143507799"^^xsd:anyURI ;
    dcat:theme legcons:Item .

F2021L00334:153 a legcons:Item,
        owl:Class,
        dcat:Resource ;
    rdfs:label "Item - I153 5 17  Prohibitions on loading"@en-AU ;
    dct:isPartOf F2021L00334:136 ;
    dct:isReferencedBy F2021L00334: ;
    rdfs:comment "5 17  Prohibitions on loading - Abrievated Graph Key: I153"@en-AU ;
    skos:definition "5 17  Prohibitions on loading"@en-AU ;
    skos:narrower F2021L00334:136 ;
    skos:prefLabel "Item I153"@en-AU ;
    dcat:accessURL <https://www.legislation.gov.au/F2021L00334/2023-08-04/2023-08-04/text/original/epub/OEBPS/document_1/document_1.html#_Toc143507800> ;
    dcat:landingPage "https://www.legislation.gov.au/F2021L00334/2023-08-04/2023-08-04/text/original/epub/OEBPS/document_1/document_1.html#_Toc143507800"^^xsd:anyURI ;
    dcat:theme legcons:Item .

F2021L00334:154 a legcons:Item,
        owl:Class,
        dcat:Resource ;
    rdfs:label "Item - I154 5 18  Container system units and equipment for loading aircraft and vessels"@en-AU ;
    dct:isPartOf F2021L00334:136 ;
    dct:isReferencedBy F2021L00334: ;
    rdfs:comment "5 18  Container system units and equipment for loading aircraft and vessels - Abrievated Graph Key: I154"@en-AU ;
    skos:definition "5 18  Container system units and equipment for loading aircraft and vessels"@en-AU ;
    skos:narrower F2021L00334:136 ;
    skos:prefLabel "Item I154"@en-AU ;
    dcat:accessURL <https://www.legislation.gov.au/F2021L00334/2023-08-04/2023-08-04/text/original/epub/OEBPS/document_1/document_1.html#_Toc143507801> ;
    dcat:landingPage "https://www.legislation.gov.au/F2021L00334/2023-08-04/2023-08-04/text/original/epub/OEBPS/document_1/document_1.html#_Toc143507801"^^xsd:anyURI ;
    dcat:theme legcons:Item .

F2021L00334:155 a legcons:Item,
        owl:Class,
        dcat:Resource ;
    rdfs:label "Item - I155 5 19  When a bolt seal must be applied to container system unit"@en-AU ;
    dct:isPartOf F2021L00334:136 ;
    dct:isReferencedBy F2021L00334: ;
    rdfs:comment "5 19  When a bolt seal must be applied to container system unit - Abrievated Graph Key: I155"@en-AU ;
    skos:definition "5 19  When a bolt seal must be applied to container system unit"@en-AU ;
    skos:narrower F2021L00334:136 ;
    skos:prefLabel "Item I155"@en-AU ;
    dcat:accessURL <https://www.legislation.gov.au/F2021L00334/2023-08-04/2023-08-04/text/original/epub/OEBPS/document_1/document_1.html#_Toc143507802> ;
    dcat:landingPage "https://www.legislation.gov.au/F2021L00334/2023-08-04/2023-08-04/text/original/epub/OEBPS/document_1/document_1.html#_Toc143507802"^^xsd:anyURI ;
    dcat:theme legcons:Item .

F2021L00334:156 a legcons:Item,
        owl:Class,
        dcat:Resource ;
    rdfs:label "Item - I156 5 20  Meat transport vehicles measuring devices and other equipment"@en-AU ;
    dct:isPartOf F2021L00334:136 ;
    dct:isReferencedBy F2021L00334: ;
    rdfs:comment "5 20  Meat transport vehicles measuring devices and other equipment - Abrievated Graph Key: I156"@en-AU ;
    skos:definition "5 20  Meat transport vehicles measuring devices and other equipment"@en-AU ;
    skos:narrower F2021L00334:136 ;
    skos:prefLabel "Item I156"@en-AU ;
    dcat:accessURL <https://www.legislation.gov.au/F2021L00334/2023-08-04/2023-08-04/text/original/epub/OEBPS/document_1/document_1.html#_Toc143507803> ;
    dcat:landingPage "https://www.legislation.gov.au/F2021L00334/2023-08-04/2023-08-04/text/original/epub/OEBPS/document_1/document_1.html#_Toc143507803"^^xsd:anyURI ;
    dcat:theme legcons:Item .

F2021L00334:157 a legcons:Subdivision,
        owl:Class,
        dcat:Resource ;
    rdfs:label "Subdivision - S157 Subdivision DTrade descriptions"@en-AU ;
    dct:isPartOf F2021L00334:136 ;
    dct:isReferencedBy F2021L00334: ;
    rdfs:comment "Subdivision DTrade descriptions - Abrievated Graph Key: S157"@en-AU ;
    skos:definition "Subdivision DTrade descriptions"@en-AU ;
    skos:narrower F2021L00334:136 ;
    skos:prefLabel "Subdivision S157"@en-AU ;
    dcat:accessURL <https://www.legislation.gov.au/F2021L00334/2023-08-04/2023-08-04/text/original/epub/OEBPS/document_1/document_1.html#_Toc143507804> ;
    dcat:landingPage "https://www.legislation.gov.au/F2021L00334/2023-08-04/2023-08-04/text/original/epub/OEBPS/document_1/document_1.html#_Toc143507804"^^xsd:anyURI ;
    dcat:theme legcons:Subdivision .

F2021L00334:158 a legcons:Item,
        owl:Class,
        dcat:Resource ;
    rdfs:label "Item - I158 5 21  Trade description must be applied to prescribed meat and meat products that are intended to be exported"@en-AU ;
    dct:isPartOf F2021L00334:136 ;
    dct:isReferencedBy F2021L00334: ;
    rdfs:comment "5 21  Trade description must be applied to prescribed meat and meat products that are intended to be exported - Abrievated Graph Key: I158"@en-AU ;
    skos:definition "5 21  Trade description must be applied to prescribed meat and meat products that are intended to be exported"@en-AU ;
    skos:narrower F2021L00334:136 ;
    skos:prefLabel "Item I158"@en-AU ;
    dcat:accessURL <https://www.legislation.gov.au/F2021L00334/2023-08-04/2023-08-04/text/original/epub/OEBPS/document_1/document_1.html#_Toc143507805> ;
    dcat:landingPage "https://www.legislation.gov.au/F2021L00334/2023-08-04/2023-08-04/text/original/epub/OEBPS/document_1/document_1.html#_Toc143507805"^^xsd:anyURI ;
    dcat:theme legcons:Item .

F2021L00334:159 a legcons:Item,
        owl:Class,
        dcat:Resource ;
    rdfs:label "Item - I159 5 22  Use of trade description Grain Fed"@en-AU ;
    dct:isPartOf F2021L00334:136 ;
    dct:isReferencedBy F2021L00334: ;
    rdfs:comment "5 22  Use of trade description Grain Fed - Abrievated Graph Key: I159"@en-AU ;
    skos:definition "5 22  Use of trade description Grain Fed"@en-AU ;
    skos:narrower F2021L00334:136 ;
    skos:prefLabel "Item I159"@en-AU ;
    dcat:accessURL <https://www.legislation.gov.au/F2021L00334/2023-08-04/2023-08-04/text/original/epub/OEBPS/document_1/document_1.html#_Toc143507806> ;
    dcat:landingPage "https://www.legislation.gov.au/F2021L00334/2023-08-04/2023-08-04/text/original/epub/OEBPS/document_1/document_1.html#_Toc143507806"^^xsd:anyURI ;
    dcat:theme legcons:Item .

F2021L00334:160 a legcons:Item,
        owl:Class,
        dcat:Resource ;
    rdfs:label "Item - I160 5 23  Prescribed meat or meat products in cartons or cans"@en-AU ;
    dct:isPartOf F2021L00334:136 ;
    dct:isReferencedBy F2021L00334: ;
    rdfs:comment "5 23  Prescribed meat or meat products in cartons or cans - Abrievated Graph Key: I160"@en-AU ;
    skos:definition "5 23  Prescribed meat or meat products in cartons or cans"@en-AU ;
    skos:narrower F2021L00334:136 ;
    skos:prefLabel "Item I160"@en-AU ;
    dcat:accessURL <https://www.legislation.gov.au/F2021L00334/2023-08-04/2023-08-04/text/original/epub/OEBPS/document_1/document_1.html#_Toc143507807> ;
    dcat:landingPage "https://www.legislation.gov.au/F2021L00334/2023-08-04/2023-08-04/text/original/epub/OEBPS/document_1/document_1.html#_Toc143507807"^^xsd:anyURI ;
    dcat:theme legcons:Item .

F2021L00334:161 a legcons:Item,
        owl:Class,
        dcat:Resource ;
    rdfs:label "Item - I161 5 24  Prescribed meat or meat products for further processing"@en-AU ;
    dct:isPartOf F2021L00334:136 ;
    dct:isReferencedBy F2021L00334: ;
    rdfs:comment "5 24  Prescribed meat or meat products for further processing - Abrievated Graph Key: I161"@en-AU ;
    skos:definition "5 24  Prescribed meat or meat products for further processing"@en-AU ;
    skos:narrower F2021L00334:136 ;
    skos:prefLabel "Item I161"@en-AU ;
    dcat:accessURL <https://www.legislation.gov.au/F2021L00334/2023-08-04/2023-08-04/text/original/epub/OEBPS/document_1/document_1.html#_Toc143507808> ;
    dcat:landingPage "https://www.legislation.gov.au/F2021L00334/2023-08-04/2023-08-04/text/original/epub/OEBPS/document_1/document_1.html#_Toc143507808"^^xsd:anyURI ;
    dcat:theme legcons:Item .

F2021L00334:162 a legcons:Subdivision,
        owl:Class,
        dcat:Resource ;
    rdfs:label "Subdivision - S162 Subdivision EOfficial marks"@en-AU ;
    dct:isPartOf F2021L00334:136 ;
    dct:isReferencedBy F2021L00334: ;
    rdfs:comment "Subdivision EOfficial marks - Abrievated Graph Key: S162"@en-AU ;
    skos:definition "Subdivision EOfficial marks"@en-AU ;
    skos:narrower F2021L00334:136 ;
    skos:prefLabel "Subdivision S162"@en-AU ;
    dcat:accessURL <https://www.legislation.gov.au/F2021L00334/2023-08-04/2023-08-04/text/original/epub/OEBPS/document_1/document_1.html#_Toc143507809> ;
    dcat:landingPage "https://www.legislation.gov.au/F2021L00334/2023-08-04/2023-08-04/text/original/epub/OEBPS/document_1/document_1.html#_Toc143507809"^^xsd:anyURI ;
    dcat:theme legcons:Subdivision .

F2021L00334:163 a legcons:Item,
        owl:Class,
        dcat:Resource ;
    rdfs:label "Item - I163 5 25  References to particular official marks"@en-AU ;
    dct:isPartOf F2021L00334:136 ;
    dct:isReferencedBy F2021L00334: ;
    rdfs:comment "5 25  References to particular official marks - Abrievated Graph Key: I163"@en-AU ;
    skos:definition "5 25  References to particular official marks"@en-AU ;
    skos:narrower F2021L00334:136 ;
    skos:prefLabel "Item I163"@en-AU ;
    dcat:accessURL <https://www.legislation.gov.au/F2021L00334/2023-08-04/2023-08-04/text/original/epub/OEBPS/document_1/document_1.html#_Toc143507810> ;
    dcat:landingPage "https://www.legislation.gov.au/F2021L00334/2023-08-04/2023-08-04/text/original/epub/OEBPS/document_1/document_1.html#_Toc143507810"^^xsd:anyURI ;
    dcat:theme legcons:Item .

F2021L00334:164 a legcons:Item,
        owl:Class,
        dcat:Resource ;
    rdfs:label "Item - I164 5 26  Carcases and carcase parts"@en-AU ;
    dct:isPartOf F2021L00334:136 ;
    dct:isReferencedBy F2021L00334: ;
    rdfs:comment "5 26  Carcases and carcase parts - Abrievated Graph Key: I164"@en-AU ;
    skos:definition "5 26  Carcases and carcase parts"@en-AU ;
    skos:narrower F2021L00334:136 ;
    skos:prefLabel "Item I164"@en-AU ;
    dcat:accessURL <https://www.legislation.gov.au/F2021L00334/2023-08-04/2023-08-04/text/original/epub/OEBPS/document_1/document_1.html#_Toc143507811> ;
    dcat:landingPage "https://www.legislation.gov.au/F2021L00334/2023-08-04/2023-08-04/text/original/epub/OEBPS/document_1/document_1.html#_Toc143507811"^^xsd:anyURI ;
    dcat:theme legcons:Item .

F2021L00334:165 a legcons:Item,
        owl:Class,
        dcat:Resource ;
    rdfs:label "Item - I165 5 27  Cartons containing prescribed meat or meat products"@en-AU ;
    dct:isPartOf F2021L00334:136 ;
    dct:isReferencedBy F2021L00334: ;
    rdfs:comment "5 27  Cartons containing prescribed meat or meat products - Abrievated Graph Key: I165"@en-AU ;
    skos:definition "5 27  Cartons containing prescribed meat or meat products"@en-AU ;
    skos:narrower F2021L00334:136 ;
    skos:prefLabel "Item I165"@en-AU ;
    dcat:accessURL <https://www.legislation.gov.au/F2021L00334/2023-08-04/2023-08-04/text/original/epub/OEBPS/document_1/document_1.html#_Toc143507812> ;
    dcat:landingPage "https://www.legislation.gov.au/F2021L00334/2023-08-04/2023-08-04/text/original/epub/OEBPS/document_1/document_1.html#_Toc143507812"^^xsd:anyURI ;
    dcat:theme legcons:Item .

F2021L00334:166 a legcons:Item,
        owl:Class,
        dcat:Resource ;
    rdfs:label "Item - I166 5 28  Cartons containing prescribed meat products that contain imported meat or meat products"@en-AU ;
    dct:isPartOf F2021L00334:136 ;
    dct:isReferencedBy F2021L00334: ;
    rdfs:comment "5 28  Cartons containing prescribed meat products that contain imported meat or meat products - Abrievated Graph Key: I166"@en-AU ;
    skos:definition "5 28  Cartons containing prescribed meat products that contain imported meat or meat products"@en-AU ;
    skos:narrower F2021L00334:136 ;
    skos:prefLabel "Item I166"@en-AU ;
    dcat:accessURL <https://www.legislation.gov.au/F2021L00334/2023-08-04/2023-08-04/text/original/epub/OEBPS/document_1/document_1.html#_Toc143507813> ;
    dcat:landingPage "https://www.legislation.gov.au/F2021L00334/2023-08-04/2023-08-04/text/original/epub/OEBPS/document_1/document_1.html#_Toc143507813"^^xsd:anyURI ;
    dcat:theme legcons:Item .

F2021L00334:167 a legcons:Item,
        owl:Class,
        dcat:Resource ;
    rdfs:label "Item - I167 5 29  Halal meat"@en-AU ;
    dct:isPartOf F2021L00334:136 ;
    dct:isReferencedBy F2021L00334: ;
    rdfs:comment "5 29  Halal meat - Abrievated Graph Key: I167"@en-AU ;
    skos:definition "5 29  Halal meat"@en-AU ;
    skos:narrower F2021L00334:136 ;
    skos:prefLabel "Item I167"@en-AU ;
    dcat:accessURL <https://www.legislation.gov.au/F2021L00334/2023-08-04/2023-08-04/text/original/epub/OEBPS/document_1/document_1.html#_Toc143507814> ;
    dcat:landingPage "https://www.legislation.gov.au/F2021L00334/2023-08-04/2023-08-04/text/original/epub/OEBPS/document_1/document_1.html#_Toc143507814"^^xsd:anyURI ;
    dcat:theme legcons:Item .

F2021L00334:168 a legcons:Item,
        owl:Class,
        dcat:Resource ;
    rdfs:label "Item - I168 5 30  State or Territory classification marks must not be applied"@en-AU ;
    dct:isPartOf F2021L00334:136 ;
    dct:isReferencedBy F2021L00334: ;
    rdfs:comment "5 30  State or Territory classification marks must not be applied - Abrievated Graph Key: I168"@en-AU ;
    skos:definition "5 30  State or Territory classification marks must not be applied"@en-AU ;
    skos:narrower F2021L00334:136 ;
    skos:prefLabel "Item I168"@en-AU ;
    dcat:accessURL <https://www.legislation.gov.au/F2021L00334/2023-08-04/2023-08-04/text/original/epub/OEBPS/document_1/document_1.html#_Toc143507815> ;
    dcat:landingPage "https://www.legislation.gov.au/F2021L00334/2023-08-04/2023-08-04/text/original/epub/OEBPS/document_1/document_1.html#_Toc143507815"^^xsd:anyURI ;
    dcat:theme legcons:Item .

F2021L00334:169 a legcons:Subdivision,
        owl:Class,
        dcat:Resource ;
    rdfs:label "Subdivision - S169 Subdivision FSegregation identification security traceability and integrity"@en-AU ;
    dct:isPartOf F2021L00334:136 ;
    dct:isReferencedBy F2021L00334: ;
    rdfs:comment "Subdivision FSegregation identification security traceability and integrity - Abrievated Graph Key: S169"@en-AU ;
    skos:definition "Subdivision FSegregation identification security traceability and integrity"@en-AU ;
    skos:narrower F2021L00334:136 ;
    skos:prefLabel "Subdivision S169"@en-AU ;
    dcat:accessURL <https://www.legislation.gov.au/F2021L00334/2023-08-04/2023-08-04/text/original/epub/OEBPS/document_1/document_1.html#_Toc143507816> ;
    dcat:landingPage "https://www.legislation.gov.au/F2021L00334/2023-08-04/2023-08-04/text/original/epub/OEBPS/document_1/document_1.html#_Toc143507816"^^xsd:anyURI ;
    dcat:theme legcons:Subdivision .

F2021L00334:17 a legcons:Item,
        owl:Class,
        dcat:Resource ;
    rdfs:label "Item - I17 2 1  Meat and meat products that are prescribed goods"@en-AU ;
    dct:isPartOf F2021L00334:16 ;
    dct:isReferencedBy F2021L00334: ;
    rdfs:comment "2 1  Meat and meat products that are prescribed goods - Abrievated Graph Key: I17"@en-AU ;
    skos:definition "2 1  Meat and meat products that are prescribed goods"@en-AU ;
    skos:narrower F2021L00334:16 ;
    skos:prefLabel "Item I17"@en-AU ;
    dcat:accessURL <https://www.legislation.gov.au/F2021L00334/2023-08-04/2023-08-04/text/original/epub/OEBPS/document_1/document_1.html#_Toc143507664> ;
    dcat:landingPage "https://www.legislation.gov.au/F2021L00334/2023-08-04/2023-08-04/text/original/epub/OEBPS/document_1/document_1.html#_Toc143507664"^^xsd:anyURI ;
    dcat:theme legcons:Item .

F2021L00334:170 a legcons:Item,
        owl:Class,
        dcat:Resource ;
    rdfs:label "Item - I170 5 31  Segregation identification security and traceabilitygeneral"@en-AU ;
    dct:isPartOf F2021L00334:136 ;
    dct:isReferencedBy F2021L00334: ;
    rdfs:comment "5 31  Segregation identification security and traceabilitygeneral - Abrievated Graph Key: I170"@en-AU ;
    skos:definition "5 31  Segregation identification security and traceabilitygeneral"@en-AU ;
    skos:narrower F2021L00334:136 ;
    skos:prefLabel "Item I170"@en-AU ;
    dcat:accessURL <https://www.legislation.gov.au/F2021L00334/2023-08-04/2023-08-04/text/original/epub/OEBPS/document_1/document_1.html#_Toc143507817> ;
    dcat:landingPage "https://www.legislation.gov.au/F2021L00334/2023-08-04/2023-08-04/text/original/epub/OEBPS/document_1/document_1.html#_Toc143507817"^^xsd:anyURI ;
    dcat:theme legcons:Item .

F2021L00334:171 a legcons:Item,
        owl:Class,
        dcat:Resource ;
    rdfs:label "Item - I171 5 32  Establishments where meat or meat products that are not for export etc are prepared"@en-AU ;
    dct:isPartOf F2021L00334:136 ;
    dct:isReferencedBy F2021L00334: ;
    rdfs:comment "5 32  Establishments where meat or meat products that are not for export etc are prepared - Abrievated Graph Key: I171"@en-AU ;
    skos:definition "5 32  Establishments where meat or meat products that are not for export etc are prepared"@en-AU ;
    skos:narrower F2021L00334:136 ;
    skos:prefLabel "Item I171"@en-AU ;
    dcat:accessURL <https://www.legislation.gov.au/F2021L00334/2023-08-04/2023-08-04/text/original/epub/OEBPS/document_1/document_1.html#_Toc143507818> ;
    dcat:landingPage "https://www.legislation.gov.au/F2021L00334/2023-08-04/2023-08-04/text/original/epub/OEBPS/document_1/document_1.html#_Toc143507818"^^xsd:anyURI ;
    dcat:theme legcons:Item .

F2021L00334:172 a legcons:Item,
        owl:Class,
        dcat:Resource ;
    rdfs:label "Item - I172 5 33  Integritygeneral"@en-AU ;
    dct:isPartOf F2021L00334:136 ;
    dct:isReferencedBy F2021L00334: ;
    rdfs:comment "5 33  Integritygeneral - Abrievated Graph Key: I172"@en-AU ;
    skos:definition "5 33  Integritygeneral"@en-AU ;
    skos:narrower F2021L00334:136 ;
    skos:prefLabel "Item I172"@en-AU ;
    dcat:accessURL <https://www.legislation.gov.au/F2021L00334/2023-08-04/2023-08-04/text/original/epub/OEBPS/document_1/document_1.html#_Toc143507819> ;
    dcat:landingPage "https://www.legislation.gov.au/F2021L00334/2023-08-04/2023-08-04/text/original/epub/OEBPS/document_1/document_1.html#_Toc143507819"^^xsd:anyURI ;
    dcat:theme legcons:Item .

F2021L00334:173 a legcons:Item,
        owl:Class,
        dcat:Resource ;
    rdfs:label "Item - I173 5 34  Identificationtype of animal"@en-AU ;
    dct:isPartOf F2021L00334:136 ;
    dct:isReferencedBy F2021L00334: ;
    rdfs:comment "5 34  Identificationtype of animal - Abrievated Graph Key: I173"@en-AU ;
    skos:definition "5 34  Identificationtype of animal"@en-AU ;
    skos:narrower F2021L00334:136 ;
    skos:prefLabel "Item I173"@en-AU ;
    dcat:accessURL <https://www.legislation.gov.au/F2021L00334/2023-08-04/2023-08-04/text/original/epub/OEBPS/document_1/document_1.html#_Toc143507820> ;
    dcat:landingPage "https://www.legislation.gov.au/F2021L00334/2023-08-04/2023-08-04/text/original/epub/OEBPS/document_1/document_1.html#_Toc143507820"^^xsd:anyURI ;
    dcat:theme legcons:Item .

F2021L00334:174 a legcons:Item,
        owl:Class,
        dcat:Resource ;
    rdfs:label "Item - I174 5 35  Integrity and identificationHalal meat"@en-AU ;
    dct:isPartOf F2021L00334:136 ;
    dct:isReferencedBy F2021L00334: ;
    rdfs:comment "5 35  Integrity and identificationHalal meat - Abrievated Graph Key: I174"@en-AU ;
    skos:definition "5 35  Integrity and identificationHalal meat"@en-AU ;
    skos:narrower F2021L00334:136 ;
    skos:prefLabel "Item I174"@en-AU ;
    dcat:accessURL <https://www.legislation.gov.au/F2021L00334/2023-08-04/2023-08-04/text/original/epub/OEBPS/document_1/document_1.html#_Toc143507821> ;
    dcat:landingPage "https://www.legislation.gov.au/F2021L00334/2023-08-04/2023-08-04/text/original/epub/OEBPS/document_1/document_1.html#_Toc143507821"^^xsd:anyURI ;
    dcat:theme legcons:Item .

F2021L00334:175 a legcons:Item,
        owl:Class,
        dcat:Resource ;
    rdfs:label "Item - I175 5 36  Export market eligibility"@en-AU ;
    dct:isPartOf F2021L00334:136 ;
    dct:isReferencedBy F2021L00334: ;
    rdfs:comment "5 36  Export market eligibility - Abrievated Graph Key: I175"@en-AU ;
    skos:definition "5 36  Export market eligibility"@en-AU ;
    skos:narrower F2021L00334:136 ;
    skos:prefLabel "Item I175"@en-AU ;
    dcat:accessURL <https://www.legislation.gov.au/F2021L00334/2023-08-04/2023-08-04/text/original/epub/OEBPS/document_1/document_1.html#_Toc143507822> ;
    dcat:landingPage "https://www.legislation.gov.au/F2021L00334/2023-08-04/2023-08-04/text/original/epub/OEBPS/document_1/document_1.html#_Toc143507822"^^xsd:anyURI ;
    dcat:theme legcons:Item .

F2021L00334:176 a legcons:Item,
        owl:Class,
        dcat:Resource ;
    rdfs:label "Item - I176 5 37  Action if prescribed meat or meat products are unwholesome or integrity etc cannot be ensured"@en-AU ;
    dct:isPartOf F2021L00334:136 ;
    dct:isReferencedBy F2021L00334: ;
    rdfs:comment "5 37  Action if prescribed meat or meat products are unwholesome or integrity etc cannot be ensured - Abrievated Graph Key: I176"@en-AU ;
    skos:definition "5 37  Action if prescribed meat or meat products are unwholesome or integrity etc cannot be ensured"@en-AU ;
    skos:narrower F2021L00334:136 ;
    skos:prefLabel "Item I176"@en-AU ;
    dcat:accessURL <https://www.legislation.gov.au/F2021L00334/2023-08-04/2023-08-04/text/original/epub/OEBPS/document_1/document_1.html#_Toc143507823> ;
    dcat:landingPage "https://www.legislation.gov.au/F2021L00334/2023-08-04/2023-08-04/text/original/epub/OEBPS/document_1/document_1.html#_Toc143507823"^^xsd:anyURI ;
    dcat:theme legcons:Item .

F2021L00334:177 a legcons:Subdivision,
        owl:Class,
        dcat:Resource ;
    rdfs:label "Subdivision - S177 Subdivision GTransfers"@en-AU ;
    dct:isPartOf F2021L00334:136 ;
    dct:isReferencedBy F2021L00334: ;
    rdfs:comment "Subdivision GTransfers - Abrievated Graph Key: S177"@en-AU ;
    skos:definition "Subdivision GTransfers"@en-AU ;
    skos:narrower F2021L00334:136 ;
    skos:prefLabel "Subdivision S177"@en-AU ;
    dcat:accessURL <https://www.legislation.gov.au/F2021L00334/2023-08-04/2023-08-04/text/original/epub/OEBPS/document_1/document_1.html#_Toc143507824> ;
    dcat:landingPage "https://www.legislation.gov.au/F2021L00334/2023-08-04/2023-08-04/text/original/epub/OEBPS/document_1/document_1.html#_Toc143507824"^^xsd:anyURI ;
    dcat:theme legcons:Subdivision .

F2021L00334:178 a legcons:Item,
        owl:Class,
        dcat:Resource ;
    rdfs:label "Item - I178 5 38  Information and declarations relating to transferred prescribed meat or meat products"@en-AU ;
    dct:isPartOf F2021L00334:136 ;
    dct:isReferencedBy F2021L00334: ;
    rdfs:comment "5 38  Information and declarations relating to transferred prescribed meat or meat products - Abrievated Graph Key: I178"@en-AU ;
    skos:definition "5 38  Information and declarations relating to transferred prescribed meat or meat products"@en-AU ;
    skos:narrower F2021L00334:136 ;
    skos:prefLabel "Item I178"@en-AU ;
    dcat:accessURL <https://www.legislation.gov.au/F2021L00334/2023-08-04/2023-08-04/text/original/epub/OEBPS/document_1/document_1.html#_Toc143507825> ;
    dcat:landingPage "https://www.legislation.gov.au/F2021L00334/2023-08-04/2023-08-04/text/original/epub/OEBPS/document_1/document_1.html#_Toc143507825"^^xsd:anyURI ;
    dcat:theme legcons:Item .

F2021L00334:179 a legcons:Item,
        owl:Class,
        dcat:Resource ;
    rdfs:label "Item - I179 5 39  Information and declarations not received or inaccurate or incomplete"@en-AU ;
    dct:isPartOf F2021L00334:136 ;
    dct:isReferencedBy F2021L00334: ;
    rdfs:comment "5 39  Information and declarations not received or inaccurate or incomplete - Abrievated Graph Key: I179"@en-AU ;
    skos:definition "5 39  Information and declarations not received or inaccurate or incomplete"@en-AU ;
    skos:narrower F2021L00334:136 ;
    skos:prefLabel "Item I179"@en-AU ;
    dcat:accessURL <https://www.legislation.gov.au/F2021L00334/2023-08-04/2023-08-04/text/original/epub/OEBPS/document_1/document_1.html#_Toc143507826> ;
    dcat:landingPage "https://www.legislation.gov.au/F2021L00334/2023-08-04/2023-08-04/text/original/epub/OEBPS/document_1/document_1.html#_Toc143507826"^^xsd:anyURI ;
    dcat:theme legcons:Item .

F2021L00334:18 a legcons:Item,
        owl:Class,
        dcat:Resource ;
    rdfs:label "Item - I18 2 2  Meat and meat products that are taken not to be prescribed goods"@en-AU ;
    dct:isPartOf F2021L00334:16 ;
    dct:isReferencedBy F2021L00334: ;
    rdfs:comment "2 2  Meat and meat products that are taken not to be prescribed goods - Abrievated Graph Key: I18"@en-AU ;
    skos:definition "2 2  Meat and meat products that are taken not to be prescribed goods"@en-AU ;
    skos:narrower F2021L00334:16 ;
    skos:prefLabel "Item I18"@en-AU ;
    dcat:accessURL <https://www.legislation.gov.au/F2021L00334/2023-08-04/2023-08-04/text/original/epub/OEBPS/document_1/document_1.html#_Toc143507665> ;
    dcat:landingPage "https://www.legislation.gov.au/F2021L00334/2023-08-04/2023-08-04/text/original/epub/OEBPS/document_1/document_1.html#_Toc143507665"^^xsd:anyURI ;
    dcat:theme legcons:Item .

F2021L00334:180 a legcons:Subdivision,
        owl:Class,
        dcat:Resource ;
    rdfs:label "Subdivision - S180 Subdivision HMeat or meat products for export to the European Union as food"@en-AU ;
    dct:isPartOf F2021L00334:136 ;
    dct:isReferencedBy F2021L00334: ;
    rdfs:comment "Subdivision HMeat or meat products for export to the European Union as food - Abrievated Graph Key: S180"@en-AU ;
    skos:definition "Subdivision HMeat or meat products for export to the European Union as food"@en-AU ;
    skos:narrower F2021L00334:136 ;
    skos:prefLabel "Subdivision S180"@en-AU ;
    dcat:accessURL <https://www.legislation.gov.au/F2021L00334/2023-08-04/2023-08-04/text/original/epub/OEBPS/document_1/document_1.html#_Toc143507827> ;
    dcat:landingPage "https://www.legislation.gov.au/F2021L00334/2023-08-04/2023-08-04/text/original/epub/OEBPS/document_1/document_1.html#_Toc143507827"^^xsd:anyURI ;
    dcat:theme legcons:Subdivision .

F2021L00334:181 a legcons:Item,
        owl:Class,
        dcat:Resource ;
    rdfs:label "Item - I181 5 40  Admission of bovine animals to registered establishment"@en-AU ;
    dct:isPartOf F2021L00334:136 ;
    dct:isReferencedBy F2021L00334: ;
    rdfs:comment "5 40  Admission of bovine animals to registered establishment - Abrievated Graph Key: I181"@en-AU ;
    skos:definition "5 40  Admission of bovine animals to registered establishment"@en-AU ;
    skos:narrower F2021L00334:136 ;
    skos:prefLabel "Item I181"@en-AU ;
    dcat:accessURL <https://www.legislation.gov.au/F2021L00334/2023-08-04/2023-08-04/text/original/epub/OEBPS/document_1/document_1.html#_Toc143507828> ;
    dcat:landingPage "https://www.legislation.gov.au/F2021L00334/2023-08-04/2023-08-04/text/original/epub/OEBPS/document_1/document_1.html#_Toc143507828"^^xsd:anyURI ;
    dcat:theme legcons:Item .

F2021L00334:182 a legcons:Item,
        owl:Class,
        dcat:Resource ;
    rdfs:label "Item - I182 5 41  Animals must be HGP free"@en-AU ;
    dct:isPartOf F2021L00334:136 ;
    dct:isReferencedBy F2021L00334: ;
    rdfs:comment "5 41  Animals must be HGP free - Abrievated Graph Key: I182"@en-AU ;
    skos:definition "5 41  Animals must be HGP free"@en-AU ;
    skos:narrower F2021L00334:136 ;
    skos:prefLabel "Item I182"@en-AU ;
    dcat:accessURL <https://www.legislation.gov.au/F2021L00334/2023-08-04/2023-08-04/text/original/epub/OEBPS/document_1/document_1.html#_Toc143507829> ;
    dcat:landingPage "https://www.legislation.gov.au/F2021L00334/2023-08-04/2023-08-04/text/original/epub/OEBPS/document_1/document_1.html#_Toc143507829"^^xsd:anyURI ;
    dcat:theme legcons:Item .

F2021L00334:183 a legcons:Item,
        owl:Class,
        dcat:Resource ;
    rdfs:label "Item - I183 5 42  Animals must be sourced from accredited property"@en-AU ;
    dct:isPartOf F2021L00334:136 ;
    dct:isReferencedBy F2021L00334: ;
    rdfs:comment "5 42  Animals must be sourced from accredited property - Abrievated Graph Key: I183"@en-AU ;
    skos:definition "5 42  Animals must be sourced from accredited property"@en-AU ;
    skos:narrower F2021L00334:136 ;
    skos:prefLabel "Item I183"@en-AU ;
    dcat:accessURL <https://www.legislation.gov.au/F2021L00334/2023-08-04/2023-08-04/text/original/epub/OEBPS/document_1/document_1.html#_Toc143507830> ;
    dcat:landingPage "https://www.legislation.gov.au/F2021L00334/2023-08-04/2023-08-04/text/original/epub/OEBPS/document_1/document_1.html#_Toc143507830"^^xsd:anyURI ;
    dcat:theme legcons:Item .

F2021L00334:184 a legcons:Subdivision,
        owl:Class,
        dcat:Resource ;
    rdfs:label "Subdivision - S184 Subdivision IMeat inspection services"@en-AU ;
    dct:isPartOf F2021L00334:136 ;
    dct:isReferencedBy F2021L00334: ;
    rdfs:comment "Subdivision IMeat inspection services - Abrievated Graph Key: S184"@en-AU ;
    skos:definition "Subdivision IMeat inspection services"@en-AU ;
    skos:narrower F2021L00334:136 ;
    skos:prefLabel "Subdivision S184"@en-AU ;
    dcat:accessURL <https://www.legislation.gov.au/F2021L00334/2023-08-04/2023-08-04/text/original/epub/OEBPS/document_1/document_1.html#_Toc143507831> ;
    dcat:landingPage "https://www.legislation.gov.au/F2021L00334/2023-08-04/2023-08-04/text/original/epub/OEBPS/document_1/document_1.html#_Toc143507831"^^xsd:anyURI ;
    dcat:theme legcons:Subdivision .

F2021L00334:185 a legcons:Item,
        owl:Class,
        dcat:Resource ;
    rdfs:label "Item - I185 5 43  Commonwealth authorised officer must be present while certain export operations are carried out"@en-AU ;
    dct:isPartOf F2021L00334:136 ;
    dct:isReferencedBy F2021L00334: ;
    rdfs:comment "5 43  Commonwealth authorised officer must be present while certain export operations are carried out - Abrievated Graph Key: I185"@en-AU ;
    skos:definition "5 43  Commonwealth authorised officer must be present while certain export operations are carried out"@en-AU ;
    skos:narrower F2021L00334:136 ;
    skos:prefLabel "Item I185"@en-AU ;
    dcat:accessURL <https://www.legislation.gov.au/F2021L00334/2023-08-04/2023-08-04/text/original/epub/OEBPS/document_1/document_1.html#_Toc143507832> ;
    dcat:landingPage "https://www.legislation.gov.au/F2021L00334/2023-08-04/2023-08-04/text/original/epub/OEBPS/document_1/document_1.html#_Toc143507832"^^xsd:anyURI ;
    dcat:theme legcons:Item .

F2021L00334:186 a legcons:Subdivision,
        owl:Class,
        dcat:Resource ;
    rdfs:label "Subdivision - S186 Subdivision JManagement practices"@en-AU ;
    dct:isPartOf F2021L00334:136 ;
    dct:isReferencedBy F2021L00334: ;
    rdfs:comment "Subdivision JManagement practices - Abrievated Graph Key: S186"@en-AU ;
    skos:definition "Subdivision JManagement practices"@en-AU ;
    skos:narrower F2021L00334:136 ;
    skos:prefLabel "Subdivision S186"@en-AU ;
    dcat:accessURL <https://www.legislation.gov.au/F2021L00334/2023-08-04/2023-08-04/text/original/epub/OEBPS/document_1/document_1.html#_Toc143507833> ;
    dcat:landingPage "https://www.legislation.gov.au/F2021L00334/2023-08-04/2023-08-04/text/original/epub/OEBPS/document_1/document_1.html#_Toc143507833"^^xsd:anyURI ;
    dcat:theme legcons:Subdivision .

F2021L00334:187 a legcons:Item,
        owl:Class,
        dcat:Resource ;
    rdfs:label "Item - I187 5 44  Management practices organisational structure resources and personnel"@en-AU ;
    dct:isPartOf F2021L00334:136 ;
    dct:isReferencedBy F2021L00334: ;
    rdfs:comment "5 44  Management practices organisational structure resources and personnel - Abrievated Graph Key: I187"@en-AU ;
    skos:definition "5 44  Management practices organisational structure resources and personnel"@en-AU ;
    skos:narrower F2021L00334:136 ;
    skos:prefLabel "Item I187"@en-AU ;
    dcat:accessURL <https://www.legislation.gov.au/F2021L00334/2023-08-04/2023-08-04/text/original/epub/OEBPS/document_1/document_1.html#_Toc143507834> ;
    dcat:landingPage "https://www.legislation.gov.au/F2021L00334/2023-08-04/2023-08-04/text/original/epub/OEBPS/document_1/document_1.html#_Toc143507834"^^xsd:anyURI ;
    dcat:theme legcons:Item .

F2021L00334:188 a legcons:Item,
        owl:Class,
        dcat:Resource ;
    rdfs:label "Item - I188 5 45  Verification of compliance with the Act and other matters"@en-AU ;
    dct:isPartOf F2021L00334:136 ;
    dct:isReferencedBy F2021L00334: ;
    rdfs:comment "5 45  Verification of compliance with the Act and other matters - Abrievated Graph Key: I188"@en-AU ;
    skos:definition "5 45  Verification of compliance with the Act and other matters"@en-AU ;
    skos:narrower F2021L00334:136 ;
    skos:prefLabel "Item I188"@en-AU ;
    dcat:accessURL <https://www.legislation.gov.au/F2021L00334/2023-08-04/2023-08-04/text/original/epub/OEBPS/document_1/document_1.html#_Toc143507835> ;
    dcat:landingPage "https://www.legislation.gov.au/F2021L00334/2023-08-04/2023-08-04/text/original/epub/OEBPS/document_1/document_1.html#_Toc143507835"^^xsd:anyURI ;
    dcat:theme legcons:Item .

F2021L00334:189 a legcons:Item,
        owl:Class,
        dcat:Resource ;
    rdfs:label "Item - I189 5 46  Action must be taken to address non compliance"@en-AU ;
    dct:isPartOf F2021L00334:136 ;
    dct:isReferencedBy F2021L00334: ;
    rdfs:comment "5 46  Action must be taken to address non compliance - Abrievated Graph Key: I189"@en-AU ;
    skos:definition "5 46  Action must be taken to address non compliance"@en-AU ;
    skos:narrower F2021L00334:136 ;
    skos:prefLabel "Item I189"@en-AU ;
    dcat:accessURL <https://www.legislation.gov.au/F2021L00334/2023-08-04/2023-08-04/text/original/epub/OEBPS/document_1/document_1.html#_Toc143507836> ;
    dcat:landingPage "https://www.legislation.gov.au/F2021L00334/2023-08-04/2023-08-04/text/original/epub/OEBPS/document_1/document_1.html#_Toc143507836"^^xsd:anyURI ;
    dcat:theme legcons:Item .

F2021L00334:190 a legcons:Item,
        owl:Class,
        dcat:Resource ;
    rdfs:label "Item - I190 5 47  Internal audit and management review"@en-AU ;
    dct:isPartOf F2021L00334:136 ;
    dct:isReferencedBy F2021L00334: ;
    rdfs:comment "5 47  Internal audit and management review - Abrievated Graph Key: I190"@en-AU ;
    skos:definition "5 47  Internal audit and management review"@en-AU ;
    skos:narrower F2021L00334:136 ;
    skos:prefLabel "Item I190"@en-AU ;
    dcat:accessURL <https://www.legislation.gov.au/F2021L00334/2023-08-04/2023-08-04/text/original/epub/OEBPS/document_1/document_1.html#_Toc143507837> ;
    dcat:landingPage "https://www.legislation.gov.au/F2021L00334/2023-08-04/2023-08-04/text/original/epub/OEBPS/document_1/document_1.html#_Toc143507837"^^xsd:anyURI ;
    dcat:theme legcons:Item .

F2021L00334:191 a legcons:Division,
        owl:Class,
        dcat:Resource ;
    rdfs:label "Division - D191 Division 3 Renewal of approved arrangement"@en-AU ;
    dct:isPartOf F2021L00334:131 ;
    dct:isReferencedBy F2021L00334: ;
    rdfs:comment "Division 3 Renewal of approved arrangement - Abrievated Graph Key: D191"@en-AU ;
    skos:definition "Division 3 Renewal of approved arrangement"@en-AU ;
    skos:narrower F2021L00334:131 ;
    skos:prefLabel "Division D191"@en-AU ;
    dcat:accessURL <https://www.legislation.gov.au/F2021L00334/2023-08-04/2023-08-04/text/original/epub/OEBPS/document_1/document_1.html#_Toc143507838> ;
    dcat:landingPage "https://www.legislation.gov.au/F2021L00334/2023-08-04/2023-08-04/text/original/epub/OEBPS/document_1/document_1.html#_Toc143507838"^^xsd:anyURI ;
    dcat:theme legcons:Division .

F2021L00334:192 a legcons:Item,
        owl:Class,
        dcat:Resource ;
    rdfs:label "Item - I192 5 48  Period within which application to renew approved arrangement must be made"@en-AU ;
    dct:isPartOf F2021L00334:131 ;
    dct:isReferencedBy F2021L00334: ;
    rdfs:comment "5 48  Period within which application to renew approved arrangement must be made - Abrievated Graph Key: I192"@en-AU ;
    skos:definition "5 48  Period within which application to renew approved arrangement must be made"@en-AU ;
    skos:narrower F2021L00334:131 ;
    skos:prefLabel "Item I192"@en-AU ;
    dcat:accessURL <https://www.legislation.gov.au/F2021L00334/2023-08-04/2023-08-04/text/original/epub/OEBPS/document_1/document_1.html#_Toc143507839> ;
    dcat:landingPage "https://www.legislation.gov.au/F2021L00334/2023-08-04/2023-08-04/text/original/epub/OEBPS/document_1/document_1.html#_Toc143507839"^^xsd:anyURI ;
    dcat:theme legcons:Item .

F2021L00334:193 a legcons:Division,
        owl:Class,
        dcat:Resource ;
    rdfs:label "Division - D193 Division 4 Variation of approved arrangement"@en-AU ;
    dct:isPartOf F2021L00334:131 ;
    dct:isReferencedBy F2021L00334: ;
    rdfs:comment "Division 4 Variation of approved arrangement - Abrievated Graph Key: D193"@en-AU ;
    skos:definition "Division 4 Variation of approved arrangement"@en-AU ;
    skos:narrower F2021L00334:131 ;
    skos:prefLabel "Division D193"@en-AU ;
    dcat:accessURL <https://www.legislation.gov.au/F2021L00334/2023-08-04/2023-08-04/text/original/epub/OEBPS/document_1/document_1.html#_Toc143507840> ;
    dcat:landingPage "https://www.legislation.gov.au/F2021L00334/2023-08-04/2023-08-04/text/original/epub/OEBPS/document_1/document_1.html#_Toc143507840"^^xsd:anyURI ;
    dcat:theme legcons:Division .

F2021L00334:195 a legcons:Item,
        owl:Class,
        dcat:Resource ;
    rdfs:label "Item - I195 5 49  Requirements that must be met for variation to be approved or conditions varied"@en-AU ;
    dct:isPartOf F2021L00334:194 ;
    dct:isReferencedBy F2021L00334: ;
    rdfs:comment "5 49  Requirements that must be met for variation to be approved or conditions varied - Abrievated Graph Key: I195"@en-AU ;
    skos:definition "5 49  Requirements that must be met for variation to be approved or conditions varied"@en-AU ;
    skos:narrower F2021L00334:194 ;
    skos:prefLabel "Item I195"@en-AU ;
    dcat:accessURL <https://www.legislation.gov.au/F2021L00334/2023-08-04/2023-08-04/text/original/epub/OEBPS/document_1/document_1.html#_Toc143507842> ;
    dcat:landingPage "https://www.legislation.gov.au/F2021L00334/2023-08-04/2023-08-04/text/original/epub/OEBPS/document_1/document_1.html#_Toc143507842"^^xsd:anyURI ;
    dcat:theme legcons:Item .

F2021L00334:196 a legcons:Item,
        owl:Class,
        dcat:Resource ;
    rdfs:label "Item - I196 5 50  Significant variations"@en-AU ;
    dct:isPartOf F2021L00334:194 ;
    dct:isReferencedBy F2021L00334: ;
    rdfs:comment "5 50  Significant variations - Abrievated Graph Key: I196"@en-AU ;
    skos:definition "5 50  Significant variations"@en-AU ;
    skos:narrower F2021L00334:194 ;
    skos:prefLabel "Item I196"@en-AU ;
    dcat:accessURL <https://www.legislation.gov.au/F2021L00334/2023-08-04/2023-08-04/text/original/epub/OEBPS/document_1/document_1.html#_Toc143507843> ;
    dcat:landingPage "https://www.legislation.gov.au/F2021L00334/2023-08-04/2023-08-04/text/original/epub/OEBPS/document_1/document_1.html#_Toc143507843"^^xsd:anyURI ;
    dcat:theme legcons:Item .

F2021L00334:198 a legcons:Item,
        owl:Class,
        dcat:Resource ;
    rdfs:label "Item - I198 5 51  Other reasons for requiring holder to vary approved arrangement"@en-AU ;
    dct:isPartOf F2021L00334:197 ;
    dct:isReferencedBy F2021L00334: ;
    rdfs:comment "5 51  Other reasons for requiring holder to vary approved arrangement - Abrievated Graph Key: I198"@en-AU ;
    skos:definition "5 51  Other reasons for requiring holder to vary approved arrangement"@en-AU ;
    skos:narrower F2021L00334:197 ;
    skos:prefLabel "Item I198"@en-AU ;
    dcat:accessURL <https://www.legislation.gov.au/F2021L00334/2023-08-04/2023-08-04/text/original/epub/OEBPS/document_1/document_1.html#_Toc143507845> ;
    dcat:landingPage "https://www.legislation.gov.au/F2021L00334/2023-08-04/2023-08-04/text/original/epub/OEBPS/document_1/document_1.html#_Toc143507845"^^xsd:anyURI ;
    dcat:theme legcons:Item .

F2021L00334:199 a legcons:Part,
        owl:Class,
        dcat:Resource ;
    rdfs:label "Part - P199 Part 2 Approved arrangements for Halal meat certification operations"@en-AU ;
    dct:isPartOf F2021L00334:130 ;
    dct:isReferencedBy F2021L00334: ;
    rdfs:comment "Part 2 Approved arrangements for Halal meat certification operations - Abrievated Graph Key: P199"@en-AU ;
    skos:definition "Part 2 Approved arrangements for Halal meat certification operations"@en-AU ;
    skos:narrower F2021L00334:130 ;
    skos:prefLabel "Part P199"@en-AU ;
    dcat:accessURL <https://www.legislation.gov.au/F2021L00334/2023-08-04/2023-08-04/text/original/epub/OEBPS/document_1/document_1.html#_Toc143507846> ;
    dcat:landingPage "https://www.legislation.gov.au/F2021L00334/2023-08-04/2023-08-04/text/original/epub/OEBPS/document_1/document_1.html#_Toc143507846"^^xsd:anyURI ;
    dcat:theme legcons:Part .

F2021L00334:2 a legcons:Part,
        owl:Class,
        dcat:Resource ;
    rdfs:label "Part - P2 Part 1 Preliminary"@en-AU ;
    dct:isPartOf F2021L00334:1 ;
    dct:isReferencedBy F2021L00334: ;
    rdfs:comment "Part 1 Preliminary - Abrievated Graph Key: P2"@en-AU ;
    skos:definition "Part 1 Preliminary"@en-AU ;
    skos:narrower F2021L00334:1 ;
    skos:prefLabel "Part P2"@en-AU ;
    dcat:accessURL <https://www.legislation.gov.au/F2021L00334/2023-08-04/2023-08-04/text/original/epub/OEBPS/document_1/document_1.html#_Toc143507649> ;
    dcat:landingPage "https://www.legislation.gov.au/F2021L00334/2023-08-04/2023-08-04/text/original/epub/OEBPS/document_1/document_1.html#_Toc143507649"^^xsd:anyURI ;
    dcat:theme legcons:Part .

F2021L00334:20 a legcons:Item,
        owl:Class,
        dcat:Resource ;
    rdfs:label "Item - I20 2 3  Purpose and application of this Division"@en-AU ;
    dct:isPartOf F2021L00334:19 ;
    dct:isReferencedBy F2021L00334: ;
    rdfs:comment "2 3  Purpose and application of this Division - Abrievated Graph Key: I20"@en-AU ;
    skos:definition "2 3  Purpose and application of this Division"@en-AU ;
    skos:narrower F2021L00334:19 ;
    skos:prefLabel "Item I20"@en-AU ;
    dcat:accessURL <https://www.legislation.gov.au/F2021L00334/2023-08-04/2023-08-04/text/original/epub/OEBPS/document_1/document_1.html#_Toc143507667> ;
    dcat:landingPage "https://www.legislation.gov.au/F2021L00334/2023-08-04/2023-08-04/text/original/epub/OEBPS/document_1/document_1.html#_Toc143507667"^^xsd:anyURI ;
    dcat:theme legcons:Item .

F2021L00334:201 a legcons:Item,
        owl:Class,
        dcat:Resource ;
    rdfs:label "Item - I201 5 52  Purpose of this Division"@en-AU ;
    dct:isPartOf F2021L00334:200 ;
    dct:isReferencedBy F2021L00334: ;
    rdfs:comment "5 52  Purpose of this Division - Abrievated Graph Key: I201"@en-AU ;
    skos:definition "5 52  Purpose of this Division"@en-AU ;
    skos:narrower F2021L00334:200 ;
    skos:prefLabel "Item I201"@en-AU ;
    dcat:accessURL <https://www.legislation.gov.au/F2021L00334/2023-08-04/2023-08-04/text/original/epub/OEBPS/document_1/document_1.html#_Toc143507848> ;
    dcat:landingPage "https://www.legislation.gov.au/F2021L00334/2023-08-04/2023-08-04/text/original/epub/OEBPS/document_1/document_1.html#_Toc143507848"^^xsd:anyURI ;
    dcat:theme legcons:Item .

F2021L00334:202 a legcons:Item,
        owl:Class,
        dcat:Resource ;
    rdfs:label "Item - I202 5 53  Other requirementsproposed arrangement for Halal meat certification operations"@en-AU ;
    dct:isPartOf F2021L00334:200 ;
    dct:isReferencedBy F2021L00334: ;
    rdfs:comment "5 53  Other requirementsproposed arrangement for Halal meat certification operations - Abrievated Graph Key: I202"@en-AU ;
    skos:definition "5 53  Other requirementsproposed arrangement for Halal meat certification operations"@en-AU ;
    skos:narrower F2021L00334:200 ;
    skos:prefLabel "Item I202"@en-AU ;
    dcat:accessURL <https://www.legislation.gov.au/F2021L00334/2023-08-04/2023-08-04/text/original/epub/OEBPS/document_1/document_1.html#_Toc143507849> ;
    dcat:landingPage "https://www.legislation.gov.au/F2021L00334/2023-08-04/2023-08-04/text/original/epub/OEBPS/document_1/document_1.html#_Toc143507849"^^xsd:anyURI ;
    dcat:theme legcons:Item .

F2021L00334:205 a legcons:Item,
        owl:Class,
        dcat:Resource ;
    rdfs:label "Item - I205 5 54  Purpose of this Division"@en-AU ;
    dct:isPartOf F2021L00334:204 ;
    dct:isReferencedBy F2021L00334: ;
    rdfs:comment "5 54  Purpose of this Division - Abrievated Graph Key: I205"@en-AU ;
    skos:definition "5 54  Purpose of this Division"@en-AU ;
    skos:narrower F2021L00334:204 ;
    skos:prefLabel "Item I205"@en-AU ;
    dcat:accessURL <https://www.legislation.gov.au/F2021L00334/2023-08-04/2023-08-04/text/original/epub/OEBPS/document_1/document_1.html#_Toc143507852> ;
    dcat:landingPage "https://www.legislation.gov.au/F2021L00334/2023-08-04/2023-08-04/text/original/epub/OEBPS/document_1/document_1.html#_Toc143507852"^^xsd:anyURI ;
    dcat:theme legcons:Item .

F2021L00334:207 a legcons:Item,
        owl:Class,
        dcat:Resource ;
    rdfs:label "Item - I207 5 55  Importing country requirements must be met"@en-AU ;
    dct:isPartOf F2021L00334:206 ;
    dct:isReferencedBy F2021L00334: ;
    rdfs:comment "5 55  Importing country requirements must be met - Abrievated Graph Key: I207"@en-AU ;
    skos:definition "5 55  Importing country requirements must be met"@en-AU ;
    skos:narrower F2021L00334:206 ;
    skos:prefLabel "Item I207"@en-AU ;
    dcat:accessURL <https://www.legislation.gov.au/F2021L00334/2023-08-04/2023-08-04/text/original/epub/OEBPS/document_1/document_1.html#_Toc143507854> ;
    dcat:landingPage "https://www.legislation.gov.au/F2021L00334/2023-08-04/2023-08-04/text/original/epub/OEBPS/document_1/document_1.html#_Toc143507854"^^xsd:anyURI ;
    dcat:theme legcons:Item .

F2021L00334:209 a legcons:Item,
        owl:Class,
        dcat:Resource ;
    rdfs:label "Item - I209 5 56  Operations must be objective fair etc and meet importing country requirements"@en-AU ;
    dct:isPartOf F2021L00334:208 ;
    dct:isReferencedBy F2021L00334: ;
    rdfs:comment "5 56  Operations must be objective fair etc and meet importing country requirements - Abrievated Graph Key: I209"@en-AU ;
    skos:definition "5 56  Operations must be objective fair etc and meet importing country requirements"@en-AU ;
    skos:narrower F2021L00334:208 ;
    skos:prefLabel "Item I209"@en-AU ;
    dcat:accessURL <https://www.legislation.gov.au/F2021L00334/2023-08-04/2023-08-04/text/original/epub/OEBPS/document_1/document_1.html#_Toc143507856> ;
    dcat:landingPage "https://www.legislation.gov.au/F2021L00334/2023-08-04/2023-08-04/text/original/epub/OEBPS/document_1/document_1.html#_Toc143507856"^^xsd:anyURI ;
    dcat:theme legcons:Item .

F2021L00334:21 a legcons:Item,
        owl:Class,
        dcat:Resource ;
    rdfs:label "Item - I21 2 4  Export of prescribed meat or meat products is prohibited unless prescribed conditions are complied with"@en-AU ;
    dct:isPartOf F2021L00334:19 ;
    dct:isReferencedBy F2021L00334: ;
    rdfs:comment "2 4  Export of prescribed meat or meat products is prohibited unless prescribed conditions are complied with - Abrievated Graph Key: I21"@en-AU ;
    skos:definition "2 4  Export of prescribed meat or meat products is prohibited unless prescribed conditions are complied with"@en-AU ;
    skos:narrower F2021L00334:19 ;
    skos:prefLabel "Item I21"@en-AU ;
    dcat:accessURL <https://www.legislation.gov.au/F2021L00334/2023-08-04/2023-08-04/text/original/epub/OEBPS/document_1/document_1.html#_Toc143507668> ;
    dcat:landingPage "https://www.legislation.gov.au/F2021L00334/2023-08-04/2023-08-04/text/original/epub/OEBPS/document_1/document_1.html#_Toc143507668"^^xsd:anyURI ;
    dcat:theme legcons:Item .

F2021L00334:210 a legcons:Item,
        owl:Class,
        dcat:Resource ;
    rdfs:label "Item - I210 5 57  Management practices organisational structure resources and personnel"@en-AU ;
    dct:isPartOf F2021L00334:208 ;
    dct:isReferencedBy F2021L00334: ;
    rdfs:comment "5 57  Management practices organisational structure resources and personnel - Abrievated Graph Key: I210"@en-AU ;
    skos:definition "5 57  Management practices organisational structure resources and personnel"@en-AU ;
    skos:narrower F2021L00334:208 ;
    skos:prefLabel "Item I210"@en-AU ;
    dcat:accessURL <https://www.legislation.gov.au/F2021L00334/2023-08-04/2023-08-04/text/original/epub/OEBPS/document_1/document_1.html#_Toc143507857> ;
    dcat:landingPage "https://www.legislation.gov.au/F2021L00334/2023-08-04/2023-08-04/text/original/epub/OEBPS/document_1/document_1.html#_Toc143507857"^^xsd:anyURI ;
    dcat:theme legcons:Item .

F2021L00334:211 a legcons:Item,
        owl:Class,
        dcat:Resource ;
    rdfs:label "Item - I211 5 58  Verification of compliance with the Act and other matters"@en-AU ;
    dct:isPartOf F2021L00334:208 ;
    dct:isReferencedBy F2021L00334: ;
    rdfs:comment "5 58  Verification of compliance with the Act and other matters - Abrievated Graph Key: I211"@en-AU ;
    skos:definition "5 58  Verification of compliance with the Act and other matters"@en-AU ;
    skos:narrower F2021L00334:208 ;
    skos:prefLabel "Item I211"@en-AU ;
    dcat:accessURL <https://www.legislation.gov.au/F2021L00334/2023-08-04/2023-08-04/text/original/epub/OEBPS/document_1/document_1.html#_Toc143507858> ;
    dcat:landingPage "https://www.legislation.gov.au/F2021L00334/2023-08-04/2023-08-04/text/original/epub/OEBPS/document_1/document_1.html#_Toc143507858"^^xsd:anyURI ;
    dcat:theme legcons:Item .

F2021L00334:212 a legcons:Item,
        owl:Class,
        dcat:Resource ;
    rdfs:label "Item - I212 5 59  Action must be taken to address non compliance"@en-AU ;
    dct:isPartOf F2021L00334:208 ;
    dct:isReferencedBy F2021L00334: ;
    rdfs:comment "5 59  Action must be taken to address non compliance - Abrievated Graph Key: I212"@en-AU ;
    skos:definition "5 59  Action must be taken to address non compliance"@en-AU ;
    skos:narrower F2021L00334:208 ;
    skos:prefLabel "Item I212"@en-AU ;
    dcat:accessURL <https://www.legislation.gov.au/F2021L00334/2023-08-04/2023-08-04/text/original/epub/OEBPS/document_1/document_1.html#_Toc143507859> ;
    dcat:landingPage "https://www.legislation.gov.au/F2021L00334/2023-08-04/2023-08-04/text/original/epub/OEBPS/document_1/document_1.html#_Toc143507859"^^xsd:anyURI ;
    dcat:theme legcons:Item .

F2021L00334:213 a legcons:Item,
        owl:Class,
        dcat:Resource ;
    rdfs:label "Item - I213 5 60  Internal audit and management review"@en-AU ;
    dct:isPartOf F2021L00334:208 ;
    dct:isReferencedBy F2021L00334: ;
    rdfs:comment "5 60  Internal audit and management review - Abrievated Graph Key: I213"@en-AU ;
    skos:definition "5 60  Internal audit and management review"@en-AU ;
    skos:narrower F2021L00334:208 ;
    skos:prefLabel "Item I213"@en-AU ;
    dcat:accessURL <https://www.legislation.gov.au/F2021L00334/2023-08-04/2023-08-04/text/original/epub/OEBPS/document_1/document_1.html#_Toc143507860> ;
    dcat:landingPage "https://www.legislation.gov.au/F2021L00334/2023-08-04/2023-08-04/text/original/epub/OEBPS/document_1/document_1.html#_Toc143507860"^^xsd:anyURI ;
    dcat:theme legcons:Item .

F2021L00334:214 a legcons:Item,
        owl:Class,
        dcat:Resource ;
    rdfs:label "Item - I214 5 61  Secretary must be notified of critical non compliance"@en-AU ;
    dct:isPartOf F2021L00334:208 ;
    dct:isReferencedBy F2021L00334: ;
    rdfs:comment "5 61  Secretary must be notified of critical non compliance - Abrievated Graph Key: I214"@en-AU ;
    skos:definition "5 61  Secretary must be notified of critical non compliance"@en-AU ;
    skos:narrower F2021L00334:208 ;
    skos:prefLabel "Item I214"@en-AU ;
    dcat:accessURL <https://www.legislation.gov.au/F2021L00334/2023-08-04/2023-08-04/text/original/epub/OEBPS/document_1/document_1.html#_Toc143507861> ;
    dcat:landingPage "https://www.legislation.gov.au/F2021L00334/2023-08-04/2023-08-04/text/original/epub/OEBPS/document_1/document_1.html#_Toc143507861"^^xsd:anyURI ;
    dcat:theme legcons:Item .

F2021L00334:216 a legcons:Item,
        owl:Class,
        dcat:Resource ;
    rdfs:label "Item - I216 5 62  Period within which application to renew approved arrangement must be made"@en-AU ;
    dct:isPartOf F2021L00334:215 ;
    dct:isReferencedBy F2021L00334: ;
    rdfs:comment "5 62  Period within which application to renew approved arrangement must be made - Abrievated Graph Key: I216"@en-AU ;
    skos:definition "5 62  Period within which application to renew approved arrangement must be made"@en-AU ;
    skos:narrower F2021L00334:215 ;
    skos:prefLabel "Item I216"@en-AU ;
    dcat:accessURL <https://www.legislation.gov.au/F2021L00334/2023-08-04/2023-08-04/text/original/epub/OEBPS/document_1/document_1.html#_Toc143507863> ;
    dcat:landingPage "https://www.legislation.gov.au/F2021L00334/2023-08-04/2023-08-04/text/original/epub/OEBPS/document_1/document_1.html#_Toc143507863"^^xsd:anyURI ;
    dcat:theme legcons:Item .

F2021L00334:219 a legcons:Item,
        owl:Class,
        dcat:Resource ;
    rdfs:label "Item - I219 5 63  Significant variations"@en-AU ;
    dct:isPartOf F2021L00334:218 ;
    dct:isReferencedBy F2021L00334: ;
    rdfs:comment "5 63  Significant variations - Abrievated Graph Key: I219"@en-AU ;
    skos:definition "5 63  Significant variations"@en-AU ;
    skos:narrower F2021L00334:218 ;
    skos:prefLabel "Item I219"@en-AU ;
    dcat:accessURL <https://www.legislation.gov.au/F2021L00334/2023-08-04/2023-08-04/text/original/epub/OEBPS/document_1/document_1.html#_Toc143507866> ;
    dcat:landingPage "https://www.legislation.gov.au/F2021L00334/2023-08-04/2023-08-04/text/original/epub/OEBPS/document_1/document_1.html#_Toc143507866"^^xsd:anyURI ;
    dcat:theme legcons:Item .

F2021L00334:221 a legcons:Item,
        owl:Class,
        dcat:Resource ;
    rdfs:label "Item - I221 5 64  Other reasons for requiring holder to vary approved arrangement"@en-AU ;
    dct:isPartOf F2021L00334:220 ;
    dct:isReferencedBy F2021L00334: ;
    rdfs:comment "5 64  Other reasons for requiring holder to vary approved arrangement - Abrievated Graph Key: I221"@en-AU ;
    skos:definition "5 64  Other reasons for requiring holder to vary approved arrangement"@en-AU ;
    skos:narrower F2021L00334:220 ;
    skos:prefLabel "Item I221"@en-AU ;
    dcat:accessURL <https://www.legislation.gov.au/F2021L00334/2023-08-04/2023-08-04/text/original/epub/OEBPS/document_1/document_1.html#_Toc143507868> ;
    dcat:landingPage "https://www.legislation.gov.au/F2021L00334/2023-08-04/2023-08-04/text/original/epub/OEBPS/document_1/document_1.html#_Toc143507868"^^xsd:anyURI ;
    dcat:theme legcons:Item .

F2021L00334:223 a legcons:Item,
        owl:Class,
        dcat:Resource ;
    rdfs:label "Item - I223 5 65  Other events of which Secretary must be notified"@en-AU ;
    dct:isPartOf F2021L00334:222 ;
    dct:isReferencedBy F2021L00334: ;
    rdfs:comment "5 65  Other events of which Secretary must be notified - Abrievated Graph Key: I223"@en-AU ;
    skos:definition "5 65  Other events of which Secretary must be notified"@en-AU ;
    skos:narrower F2021L00334:222 ;
    skos:prefLabel "Item I223"@en-AU ;
    dcat:accessURL <https://www.legislation.gov.au/F2021L00334/2023-08-04/2023-08-04/text/original/epub/OEBPS/document_1/document_1.html#_Toc143507870> ;
    dcat:landingPage "https://www.legislation.gov.au/F2021L00334/2023-08-04/2023-08-04/text/original/epub/OEBPS/document_1/document_1.html#_Toc143507870"^^xsd:anyURI ;
    dcat:theme legcons:Item .

F2021L00334:225 a legcons:Item,
        owl:Class,
        dcat:Resource ;
    rdfs:label "Item - I225 5 66  Kinds of persons who are required to be fit and proper persons"@en-AU ;
    dct:isPartOf F2021L00334:224 ;
    dct:isReferencedBy F2021L00334: ;
    rdfs:comment "5 66  Kinds of persons who are required to be fit and proper persons - Abrievated Graph Key: I225"@en-AU ;
    skos:definition "5 66  Kinds of persons who are required to be fit and proper persons"@en-AU ;
    skos:narrower F2021L00334:224 ;
    skos:prefLabel "Item I225"@en-AU ;
    dcat:accessURL <https://www.legislation.gov.au/F2021L00334/2023-08-04/2023-08-04/text/original/epub/OEBPS/document_1/document_1.html#_Toc143507872> ;
    dcat:landingPage "https://www.legislation.gov.au/F2021L00334/2023-08-04/2023-08-04/text/original/epub/OEBPS/document_1/document_1.html#_Toc143507872"^^xsd:anyURI ;
    dcat:theme legcons:Item .

F2021L00334:226 a legcons:Part,
        owl:Class,
        dcat:Resource ;
    rdfs:label "Part - P226 Part 3 Matters relating to applications"@en-AU ;
    dct:isPartOf F2021L00334:130 ;
    dct:isReferencedBy F2021L00334: ;
    rdfs:comment "Part 3 Matters relating to applications - Abrievated Graph Key: P226"@en-AU ;
    skos:definition "Part 3 Matters relating to applications"@en-AU ;
    skos:narrower F2021L00334:130 ;
    skos:prefLabel "Part P226"@en-AU ;
    dcat:accessURL <https://www.legislation.gov.au/F2021L00334/2023-08-04/2023-08-04/text/original/epub/OEBPS/document_1/document_1.html#_Toc143507873> ;
    dcat:landingPage "https://www.legislation.gov.au/F2021L00334/2023-08-04/2023-08-04/text/original/epub/OEBPS/document_1/document_1.html#_Toc143507873"^^xsd:anyURI ;
    dcat:theme legcons:Part .

F2021L00334:227 a legcons:Item,
        owl:Class,
        dcat:Resource ;
    rdfs:label "Item - I227 5 67  Application of this Part"@en-AU ;
    dct:isPartOf F2021L00334:130 ;
    dct:isReferencedBy F2021L00334: ;
    rdfs:comment "5 67  Application of this Part - Abrievated Graph Key: I227"@en-AU ;
    skos:definition "5 67  Application of this Part"@en-AU ;
    skos:narrower F2021L00334:130 ;
    skos:prefLabel "Item I227"@en-AU ;
    dcat:accessURL <https://www.legislation.gov.au/F2021L00334/2023-08-04/2023-08-04/text/original/epub/OEBPS/document_1/document_1.html#_Toc143507874> ;
    dcat:landingPage "https://www.legislation.gov.au/F2021L00334/2023-08-04/2023-08-04/text/original/epub/OEBPS/document_1/document_1.html#_Toc143507874"^^xsd:anyURI ;
    dcat:theme legcons:Item .

F2021L00334:228 a legcons:Item,
        owl:Class,
        dcat:Resource ;
    rdfs:label "Item - I228 5 68  Documents to accompany application relating to Halal meat certification operations"@en-AU ;
    dct:isPartOf F2021L00334:130 ;
    dct:isReferencedBy F2021L00334: ;
    rdfs:comment "5 68  Documents to accompany application relating to Halal meat certification operations - Abrievated Graph Key: I228"@en-AU ;
    skos:definition "5 68  Documents to accompany application relating to Halal meat certification operations"@en-AU ;
    skos:narrower F2021L00334:130 ;
    skos:prefLabel "Item I228"@en-AU ;
    dcat:accessURL <https://www.legislation.gov.au/F2021L00334/2023-08-04/2023-08-04/text/original/epub/OEBPS/document_1/document_1.html#_Toc143507875> ;
    dcat:landingPage "https://www.legislation.gov.au/F2021L00334/2023-08-04/2023-08-04/text/original/epub/OEBPS/document_1/document_1.html#_Toc143507875"^^xsd:anyURI ;
    dcat:theme legcons:Item .

F2021L00334:229 a legcons:Item,
        owl:Class,
        dcat:Resource ;
    rdfs:label "Item - I229 5 69  Initial consideration period"@en-AU ;
    dct:isPartOf F2021L00334:130 ;
    dct:isReferencedBy F2021L00334: ;
    rdfs:comment "5 69  Initial consideration period - Abrievated Graph Key: I229"@en-AU ;
    skos:definition "5 69  Initial consideration period"@en-AU ;
    skos:narrower F2021L00334:130 ;
    skos:prefLabel "Item I229"@en-AU ;
    dcat:accessURL <https://www.legislation.gov.au/F2021L00334/2023-08-04/2023-08-04/text/original/epub/OEBPS/document_1/document_1.html#_Toc143507876> ;
    dcat:landingPage "https://www.legislation.gov.au/F2021L00334/2023-08-04/2023-08-04/text/original/epub/OEBPS/document_1/document_1.html#_Toc143507876"^^xsd:anyURI ;
    dcat:theme legcons:Item .

F2021L00334:23 a legcons:Item,
        owl:Class,
        dcat:Resource ;
    rdfs:label "Item - I23 2 5  Application of this Part"@en-AU ;
    dct:isPartOf F2021L00334:22 ;
    dct:isReferencedBy F2021L00334: ;
    rdfs:comment "2 5  Application of this Part - Abrievated Graph Key: I23"@en-AU ;
    skos:definition "2 5  Application of this Part"@en-AU ;
    skos:narrower F2021L00334:22 ;
    skos:prefLabel "Item I23"@en-AU ;
    dcat:accessURL <https://www.legislation.gov.au/F2021L00334/2023-08-04/2023-08-04/text/original/epub/OEBPS/document_1/document_1.html#_Toc143507670> ;
    dcat:landingPage "https://www.legislation.gov.au/F2021L00334/2023-08-04/2023-08-04/text/original/epub/OEBPS/document_1/document_1.html#_Toc143507670"^^xsd:anyURI ;
    dcat:theme legcons:Item .

F2021L00334:230 a legcons:Item,
        owl:Class,
        dcat:Resource ;
    rdfs:label "Item - I230 5 70  Period within which request relating to application must be complied with"@en-AU ;
    dct:isPartOf F2021L00334:130 ;
    dct:isReferencedBy F2021L00334: ;
    rdfs:comment "5 70  Period within which request relating to application must be complied with - Abrievated Graph Key: I230"@en-AU ;
    skos:definition "5 70  Period within which request relating to application must be complied with"@en-AU ;
    skos:narrower F2021L00334:130 ;
    skos:prefLabel "Item I230"@en-AU ;
    dcat:accessURL <https://www.legislation.gov.au/F2021L00334/2023-08-04/2023-08-04/text/original/epub/OEBPS/document_1/document_1.html#_Toc143507877> ;
    dcat:landingPage "https://www.legislation.gov.au/F2021L00334/2023-08-04/2023-08-04/text/original/epub/OEBPS/document_1/document_1.html#_Toc143507877"^^xsd:anyURI ;
    dcat:theme legcons:Item .

F2021L00334:233 a legcons:Item,
        owl:Class,
        dcat:Resource ;
    rdfs:label "Item - I233 6 1  Other requirements that must be met for meat export licence to be granted"@en-AU ;
    dct:isPartOf F2021L00334:232 ;
    dct:isReferencedBy F2021L00334: ;
    rdfs:comment "6 1  Other requirements that must be met for meat export licence to be granted - Abrievated Graph Key: I233"@en-AU ;
    skos:definition "6 1  Other requirements that must be met for meat export licence to be granted"@en-AU ;
    skos:narrower F2021L00334:232 ;
    skos:prefLabel "Item I233"@en-AU ;
    dcat:accessURL <https://www.legislation.gov.au/F2021L00334/2023-08-04/2023-08-04/text/original/epub/OEBPS/document_1/document_1.html#_Toc143507880> ;
    dcat:landingPage "https://www.legislation.gov.au/F2021L00334/2023-08-04/2023-08-04/text/original/epub/OEBPS/document_1/document_1.html#_Toc143507880"^^xsd:anyURI ;
    dcat:theme legcons:Item .

F2021L00334:235 a legcons:Item,
        owl:Class,
        dcat:Resource ;
    rdfs:label "Item - I235 6 2  Condition of meat export licence"@en-AU ;
    dct:isPartOf F2021L00334:234 ;
    dct:isReferencedBy F2021L00334: ;
    rdfs:comment "6 2  Condition of meat export licence - Abrievated Graph Key: I235"@en-AU ;
    skos:definition "6 2  Condition of meat export licence"@en-AU ;
    skos:narrower F2021L00334:234 ;
    skos:prefLabel "Item I235"@en-AU ;
    dcat:accessURL <https://www.legislation.gov.au/F2021L00334/2023-08-04/2023-08-04/text/original/epub/OEBPS/document_1/document_1.html#_Toc143507882> ;
    dcat:landingPage "https://www.legislation.gov.au/F2021L00334/2023-08-04/2023-08-04/text/original/epub/OEBPS/document_1/document_1.html#_Toc143507882"^^xsd:anyURI ;
    dcat:theme legcons:Item .

F2021L00334:237 a legcons:Item,
        owl:Class,
        dcat:Resource ;
    rdfs:label "Item - I237 6 3  Period within which application to renew meat export licence must be made"@en-AU ;
    dct:isPartOf F2021L00334:236 ;
    dct:isReferencedBy F2021L00334: ;
    rdfs:comment "6 3  Period within which application to renew meat export licence must be made - Abrievated Graph Key: I237"@en-AU ;
    skos:definition "6 3  Period within which application to renew meat export licence must be made"@en-AU ;
    skos:narrower F2021L00334:236 ;
    skos:prefLabel "Item I237"@en-AU ;
    dcat:accessURL <https://www.legislation.gov.au/F2021L00334/2023-08-04/2023-08-04/text/original/epub/OEBPS/document_1/document_1.html#_Toc143507884> ;
    dcat:landingPage "https://www.legislation.gov.au/F2021L00334/2023-08-04/2023-08-04/text/original/epub/OEBPS/document_1/document_1.html#_Toc143507884"^^xsd:anyURI ;
    dcat:theme legcons:Item .

F2021L00334:239 a legcons:Item,
        owl:Class,
        dcat:Resource ;
    rdfs:label "Item - I239 6 4  Other grounds for suspension"@en-AU ;
    dct:isPartOf F2021L00334:238 ;
    dct:isReferencedBy F2021L00334: ;
    rdfs:comment "6 4  Other grounds for suspension - Abrievated Graph Key: I239"@en-AU ;
    skos:definition "6 4  Other grounds for suspension"@en-AU ;
    skos:narrower F2021L00334:238 ;
    skos:prefLabel "Item I239"@en-AU ;
    dcat:accessURL <https://www.legislation.gov.au/F2021L00334/2023-08-04/2023-08-04/text/original/epub/OEBPS/document_1/document_1.html#_Toc143507886> ;
    dcat:landingPage "https://www.legislation.gov.au/F2021L00334/2023-08-04/2023-08-04/text/original/epub/OEBPS/document_1/document_1.html#_Toc143507886"^^xsd:anyURI ;
    dcat:theme legcons:Item .

F2021L00334:24 a legcons:Item,
        owl:Class,
        dcat:Resource ;
    rdfs:label "Item - I24 2 6  Period for making application for exemption"@en-AU ;
    dct:isPartOf F2021L00334:22 ;
    dct:isReferencedBy F2021L00334: ;
    rdfs:comment "2 6  Period for making application for exemption - Abrievated Graph Key: I24"@en-AU ;
    skos:definition "2 6  Period for making application for exemption"@en-AU ;
    skos:narrower F2021L00334:22 ;
    skos:prefLabel "Item I24"@en-AU ;
    dcat:accessURL <https://www.legislation.gov.au/F2021L00334/2023-08-04/2023-08-04/text/original/epub/OEBPS/document_1/document_1.html#_Toc143507671> ;
    dcat:landingPage "https://www.legislation.gov.au/F2021L00334/2023-08-04/2023-08-04/text/original/epub/OEBPS/document_1/document_1.html#_Toc143507671"^^xsd:anyURI ;
    dcat:theme legcons:Item .

F2021L00334:241 a legcons:Item,
        owl:Class,
        dcat:Resource ;
    rdfs:label "Item - I241 6 5  Other grounds for revocation"@en-AU ;
    dct:isPartOf F2021L00334:240 ;
    dct:isReferencedBy F2021L00334: ;
    rdfs:comment "6 5  Other grounds for revocation - Abrievated Graph Key: I241"@en-AU ;
    skos:definition "6 5  Other grounds for revocation"@en-AU ;
    skos:narrower F2021L00334:240 ;
    skos:prefLabel "Item I241"@en-AU ;
    dcat:accessURL <https://www.legislation.gov.au/F2021L00334/2023-08-04/2023-08-04/text/original/epub/OEBPS/document_1/document_1.html#_Toc143507888> ;
    dcat:landingPage "https://www.legislation.gov.au/F2021L00334/2023-08-04/2023-08-04/text/original/epub/OEBPS/document_1/document_1.html#_Toc143507888"^^xsd:anyURI ;
    dcat:theme legcons:Item .

F2021L00334:243 a legcons:Item,
        owl:Class,
        dcat:Resource ;
    rdfs:label "Item - I243 6 6  Other events of which Secretary must be notified"@en-AU ;
    dct:isPartOf F2021L00334:242 ;
    dct:isReferencedBy F2021L00334: ;
    rdfs:comment "6 6  Other events of which Secretary must be notified - Abrievated Graph Key: I243"@en-AU ;
    skos:definition "6 6  Other events of which Secretary must be notified"@en-AU ;
    skos:narrower F2021L00334:242 ;
    skos:prefLabel "Item I243"@en-AU ;
    dcat:accessURL <https://www.legislation.gov.au/F2021L00334/2023-08-04/2023-08-04/text/original/epub/OEBPS/document_1/document_1.html#_Toc143507890> ;
    dcat:landingPage "https://www.legislation.gov.au/F2021L00334/2023-08-04/2023-08-04/text/original/epub/OEBPS/document_1/document_1.html#_Toc143507890"^^xsd:anyURI ;
    dcat:theme legcons:Item .

F2021L00334:245 a legcons:Item,
        owl:Class,
        dcat:Resource ;
    rdfs:label "Item - I245 6 7  Kinds of persons who are required to be fit and proper persons"@en-AU ;
    dct:isPartOf F2021L00334:244 ;
    dct:isReferencedBy F2021L00334: ;
    rdfs:comment "6 7  Kinds of persons who are required to be fit and proper persons - Abrievated Graph Key: I245"@en-AU ;
    skos:definition "6 7  Kinds of persons who are required to be fit and proper persons"@en-AU ;
    skos:narrower F2021L00334:244 ;
    skos:prefLabel "Item I245"@en-AU ;
    dcat:accessURL <https://www.legislation.gov.au/F2021L00334/2023-08-04/2023-08-04/text/original/epub/OEBPS/document_1/document_1.html#_Toc143507892> ;
    dcat:landingPage "https://www.legislation.gov.au/F2021L00334/2023-08-04/2023-08-04/text/original/epub/OEBPS/document_1/document_1.html#_Toc143507892"^^xsd:anyURI ;
    dcat:theme legcons:Item .

F2021L00334:247 a legcons:Item,
        owl:Class,
        dcat:Resource ;
    rdfs:label "Item - I247 6 8  Application of this Part"@en-AU ;
    dct:isPartOf F2021L00334:246 ;
    dct:isReferencedBy F2021L00334: ;
    rdfs:comment "6 8  Application of this Part - Abrievated Graph Key: I247"@en-AU ;
    skos:definition "6 8  Application of this Part"@en-AU ;
    skos:narrower F2021L00334:246 ;
    skos:prefLabel "Item I247"@en-AU ;
    dcat:accessURL <https://www.legislation.gov.au/F2021L00334/2023-08-04/2023-08-04/text/original/epub/OEBPS/document_1/document_1.html#_Toc143507894> ;
    dcat:landingPage "https://www.legislation.gov.au/F2021L00334/2023-08-04/2023-08-04/text/original/epub/OEBPS/document_1/document_1.html#_Toc143507894"^^xsd:anyURI ;
    dcat:theme legcons:Item .

F2021L00334:248 a legcons:Item,
        owl:Class,
        dcat:Resource ;
    rdfs:label "Item - I248 6 9  Documents to accompany application"@en-AU ;
    dct:isPartOf F2021L00334:246 ;
    dct:isReferencedBy F2021L00334: ;
    rdfs:comment "6 9  Documents to accompany application - Abrievated Graph Key: I248"@en-AU ;
    skos:definition "6 9  Documents to accompany application"@en-AU ;
    skos:narrower F2021L00334:246 ;
    skos:prefLabel "Item I248"@en-AU ;
    dcat:accessURL <https://www.legislation.gov.au/F2021L00334/2023-08-04/2023-08-04/text/original/epub/OEBPS/document_1/document_1.html#_Toc143507895> ;
    dcat:landingPage "https://www.legislation.gov.au/F2021L00334/2023-08-04/2023-08-04/text/original/epub/OEBPS/document_1/document_1.html#_Toc143507895"^^xsd:anyURI ;
    dcat:theme legcons:Item .

F2021L00334:249 a legcons:Item,
        owl:Class,
        dcat:Resource ;
    rdfs:label "Item - I249 6 10  Initial consideration period"@en-AU ;
    dct:isPartOf F2021L00334:246 ;
    dct:isReferencedBy F2021L00334: ;
    rdfs:comment "6 10  Initial consideration period - Abrievated Graph Key: I249"@en-AU ;
    skos:definition "6 10  Initial consideration period"@en-AU ;
    skos:narrower F2021L00334:246 ;
    skos:prefLabel "Item I249"@en-AU ;
    dcat:accessURL <https://www.legislation.gov.au/F2021L00334/2023-08-04/2023-08-04/text/original/epub/OEBPS/document_1/document_1.html#_Toc143507896> ;
    dcat:landingPage "https://www.legislation.gov.au/F2021L00334/2023-08-04/2023-08-04/text/original/epub/OEBPS/document_1/document_1.html#_Toc143507896"^^xsd:anyURI ;
    dcat:theme legcons:Item .

F2021L00334:25 a legcons:Item,
        owl:Class,
        dcat:Resource ;
    rdfs:label "Item - I25 2 7  Conditions of exemptionmatters to which Secretary must have regard"@en-AU ;
    dct:isPartOf F2021L00334:22 ;
    dct:isReferencedBy F2021L00334: ;
    rdfs:comment "2 7  Conditions of exemptionmatters to which Secretary must have regard - Abrievated Graph Key: I25"@en-AU ;
    skos:definition "2 7  Conditions of exemptionmatters to which Secretary must have regard"@en-AU ;
    skos:narrower F2021L00334:22 ;
    skos:prefLabel "Item I25"@en-AU ;
    dcat:accessURL <https://www.legislation.gov.au/F2021L00334/2023-08-04/2023-08-04/text/original/epub/OEBPS/document_1/document_1.html#_Toc143507672> ;
    dcat:landingPage "https://www.legislation.gov.au/F2021L00334/2023-08-04/2023-08-04/text/original/epub/OEBPS/document_1/document_1.html#_Toc143507672"^^xsd:anyURI ;
    dcat:theme legcons:Item .

F2021L00334:250 a legcons:Item,
        owl:Class,
        dcat:Resource ;
    rdfs:label "Item - I250 6 11  Period within which request relating to application must be complied with"@en-AU ;
    dct:isPartOf F2021L00334:246 ;
    dct:isReferencedBy F2021L00334: ;
    rdfs:comment "6 11  Period within which request relating to application must be complied with - Abrievated Graph Key: I250"@en-AU ;
    skos:definition "6 11  Period within which request relating to application must be complied with"@en-AU ;
    skos:narrower F2021L00334:246 ;
    skos:prefLabel "Item I250"@en-AU ;
    dcat:accessURL <https://www.legislation.gov.au/F2021L00334/2023-08-04/2023-08-04/text/original/epub/OEBPS/document_1/document_1.html#_Toc143507897> ;
    dcat:landingPage "https://www.legislation.gov.au/F2021L00334/2023-08-04/2023-08-04/text/original/epub/OEBPS/document_1/document_1.html#_Toc143507897"^^xsd:anyURI ;
    dcat:theme legcons:Item .

F2021L00334:253 a legcons:Item,
        owl:Class,
        dcat:Resource ;
    rdfs:label "Item - I253 7 1  Period of effect of export permit"@en-AU ;
    dct:isPartOf F2021L00334:252 ;
    dct:isReferencedBy F2021L00334: ;
    rdfs:comment "7 1  Period of effect of export permit - Abrievated Graph Key: I253"@en-AU ;
    skos:definition "7 1  Period of effect of export permit"@en-AU ;
    skos:narrower F2021L00334:252 ;
    skos:prefLabel "Item I253"@en-AU ;
    dcat:accessURL <https://www.legislation.gov.au/F2021L00334/2023-08-04/2023-08-04/text/original/epub/OEBPS/document_1/document_1.html#_Toc143507900> ;
    dcat:landingPage "https://www.legislation.gov.au/F2021L00334/2023-08-04/2023-08-04/text/original/epub/OEBPS/document_1/document_1.html#_Toc143507900"^^xsd:anyURI ;
    dcat:theme legcons:Item .

F2021L00334:255 a legcons:Item,
        owl:Class,
        dcat:Resource ;
    rdfs:label "Item - I255 7 2  Period of effect of varied export permit"@en-AU ;
    dct:isPartOf F2021L00334:254 ;
    dct:isReferencedBy F2021L00334: ;
    rdfs:comment "7 2  Period of effect of varied export permit - Abrievated Graph Key: I255"@en-AU ;
    skos:definition "7 2  Period of effect of varied export permit"@en-AU ;
    skos:narrower F2021L00334:254 ;
    skos:prefLabel "Item I255"@en-AU ;
    dcat:accessURL <https://www.legislation.gov.au/F2021L00334/2023-08-04/2023-08-04/text/original/epub/OEBPS/document_1/document_1.html#_Toc143507902> ;
    dcat:landingPage "https://www.legislation.gov.au/F2021L00334/2023-08-04/2023-08-04/text/original/epub/OEBPS/document_1/document_1.html#_Toc143507902"^^xsd:anyURI ;
    dcat:theme legcons:Item .

F2021L00334:256 a legcons:Item,
        owl:Class,
        dcat:Resource ;
    rdfs:label "Item - I256 7 3  Circumstances in which export permit may be suspended"@en-AU ;
    dct:isPartOf F2021L00334:254 ;
    dct:isReferencedBy F2021L00334: ;
    rdfs:comment "7 3  Circumstances in which export permit may be suspended - Abrievated Graph Key: I256"@en-AU ;
    skos:definition "7 3  Circumstances in which export permit may be suspended"@en-AU ;
    skos:narrower F2021L00334:254 ;
    skos:prefLabel "Item I256"@en-AU ;
    dcat:accessURL <https://www.legislation.gov.au/F2021L00334/2023-08-04/2023-08-04/text/original/epub/OEBPS/document_1/document_1.html#_Toc143507903> ;
    dcat:landingPage "https://www.legislation.gov.au/F2021L00334/2023-08-04/2023-08-04/text/original/epub/OEBPS/document_1/document_1.html#_Toc143507903"^^xsd:anyURI ;
    dcat:theme legcons:Item .

F2021L00334:257 a legcons:Item,
        owl:Class,
        dcat:Resource ;
    rdfs:label "Item - I257 7 4  Other circumstances in which export permit may be revoked"@en-AU ;
    dct:isPartOf F2021L00334:254 ;
    dct:isReferencedBy F2021L00334: ;
    rdfs:comment "7 4  Other circumstances in which export permit may be revoked - Abrievated Graph Key: I257"@en-AU ;
    skos:definition "7 4  Other circumstances in which export permit may be revoked"@en-AU ;
    skos:narrower F2021L00334:254 ;
    skos:prefLabel "Item I257"@en-AU ;
    dcat:accessURL <https://www.legislation.gov.au/F2021L00334/2023-08-04/2023-08-04/text/original/epub/OEBPS/document_1/document_1.html#_Toc143507904> ;
    dcat:landingPage "https://www.legislation.gov.au/F2021L00334/2023-08-04/2023-08-04/text/original/epub/OEBPS/document_1/document_1.html#_Toc143507904"^^xsd:anyURI ;
    dcat:theme legcons:Item .

F2021L00334:259 a legcons:Item,
        owl:Class,
        dcat:Resource ;
    rdfs:label "Item - I259 7 5  Changes that require additional or corrected information to be given to the Secretary"@en-AU ;
    dct:isPartOf F2021L00334:258 ;
    dct:isReferencedBy F2021L00334: ;
    rdfs:comment "7 5  Changes that require additional or corrected information to be given to the Secretary - Abrievated Graph Key: I259"@en-AU ;
    skos:definition "7 5  Changes that require additional or corrected information to be given to the Secretary"@en-AU ;
    skos:narrower F2021L00334:258 ;
    skos:prefLabel "Item I259"@en-AU ;
    dcat:accessURL <https://www.legislation.gov.au/F2021L00334/2023-08-04/2023-08-04/text/original/epub/OEBPS/document_1/document_1.html#_Toc143507906> ;
    dcat:landingPage "https://www.legislation.gov.au/F2021L00334/2023-08-04/2023-08-04/text/original/epub/OEBPS/document_1/document_1.html#_Toc143507906"^^xsd:anyURI ;
    dcat:theme legcons:Item .

F2021L00334:26 a legcons:Item,
        owl:Class,
        dcat:Resource ;
    rdfs:label "Item - I26 2 8  Period of effect of exemption"@en-AU ;
    dct:isPartOf F2021L00334:22 ;
    dct:isReferencedBy F2021L00334: ;
    rdfs:comment "2 8  Period of effect of exemption - Abrievated Graph Key: I26"@en-AU ;
    skos:definition "2 8  Period of effect of exemption"@en-AU ;
    skos:narrower F2021L00334:22 ;
    skos:prefLabel "Item I26"@en-AU ;
    dcat:accessURL <https://www.legislation.gov.au/F2021L00334/2023-08-04/2023-08-04/text/original/epub/OEBPS/document_1/document_1.html#_Toc143507673> ;
    dcat:landingPage "https://www.legislation.gov.au/F2021L00334/2023-08-04/2023-08-04/text/original/epub/OEBPS/document_1/document_1.html#_Toc143507673"^^xsd:anyURI ;
    dcat:theme legcons:Item .

F2021L00334:260 a legcons:Item,
        owl:Class,
        dcat:Resource ;
    rdfs:label "Item - I260 7 6  Return of export permit"@en-AU ;
    dct:isPartOf F2021L00334:258 ;
    dct:isReferencedBy F2021L00334: ;
    rdfs:comment "7 6  Return of export permit - Abrievated Graph Key: I260"@en-AU ;
    skos:definition "7 6  Return of export permit"@en-AU ;
    skos:narrower F2021L00334:258 ;
    skos:prefLabel "Item I260"@en-AU ;
    dcat:accessURL <https://www.legislation.gov.au/F2021L00334/2023-08-04/2023-08-04/text/original/epub/OEBPS/document_1/document_1.html#_Toc143507907> ;
    dcat:landingPage "https://www.legislation.gov.au/F2021L00334/2023-08-04/2023-08-04/text/original/epub/OEBPS/document_1/document_1.html#_Toc143507907"^^xsd:anyURI ;
    dcat:theme legcons:Item .

F2021L00334:261 a legcons:Item,
        owl:Class,
        dcat:Resource ;
    rdfs:label "Item - I261 7 7  Notification that prescribed meat or meat products are not to be exported"@en-AU ;
    dct:isPartOf F2021L00334:258 ;
    dct:isReferencedBy F2021L00334: ;
    rdfs:comment "7 7  Notification that prescribed meat or meat products are not to be exported - Abrievated Graph Key: I261"@en-AU ;
    skos:definition "7 7  Notification that prescribed meat or meat products are not to be exported"@en-AU ;
    skos:narrower F2021L00334:258 ;
    skos:prefLabel "Item I261"@en-AU ;
    dcat:accessURL <https://www.legislation.gov.au/F2021L00334/2023-08-04/2023-08-04/text/original/epub/OEBPS/document_1/document_1.html#_Toc143507908> ;
    dcat:landingPage "https://www.legislation.gov.au/F2021L00334/2023-08-04/2023-08-04/text/original/epub/OEBPS/document_1/document_1.html#_Toc143507908"^^xsd:anyURI ;
    dcat:theme legcons:Item .

F2021L00334:262 a legcons:Item,
        owl:Class,
        dcat:Resource ;
    rdfs:label "Item - I262 7 8  Application for export permit must include declaration"@en-AU ;
    dct:isPartOf F2021L00334:258 ;
    dct:isReferencedBy F2021L00334: ;
    rdfs:comment "7 8  Application for export permit must include declaration - Abrievated Graph Key: I262"@en-AU ;
    skos:definition "7 8  Application for export permit must include declaration"@en-AU ;
    skos:narrower F2021L00334:258 ;
    skos:prefLabel "Item I262"@en-AU ;
    dcat:accessURL <https://www.legislation.gov.au/F2021L00334/2023-08-04/2023-08-04/text/original/epub/OEBPS/document_1/document_1.html#_Toc143507909> ;
    dcat:landingPage "https://www.legislation.gov.au/F2021L00334/2023-08-04/2023-08-04/text/original/epub/OEBPS/document_1/document_1.html#_Toc143507909"^^xsd:anyURI ;
    dcat:theme legcons:Item .

F2021L00334:265 a legcons:Item,
        owl:Class,
        dcat:Resource ;
    rdfs:label "Item - I265 8 1  Information to be included in notice of intention to export"@en-AU ;
    dct:isPartOf F2021L00334:264 ;
    dct:isReferencedBy F2021L00334: ;
    rdfs:comment "8 1  Information to be included in notice of intention to export - Abrievated Graph Key: I265"@en-AU ;
    skos:definition "8 1  Information to be included in notice of intention to export"@en-AU ;
    skos:narrower F2021L00334:264 ;
    skos:prefLabel "Item I265"@en-AU ;
    dcat:accessURL <https://www.legislation.gov.au/F2021L00334/2023-08-04/2023-08-04/text/original/epub/OEBPS/document_1/document_1.html#_Toc143507912> ;
    dcat:landingPage "https://www.legislation.gov.au/F2021L00334/2023-08-04/2023-08-04/text/original/epub/OEBPS/document_1/document_1.html#_Toc143507912"^^xsd:anyURI ;
    dcat:theme legcons:Item .

F2021L00334:266 a legcons:Item,
        owl:Class,
        dcat:Resource ;
    rdfs:label "Item - I266 8 2  Person who must give notice of intention to export"@en-AU ;
    dct:isPartOf F2021L00334:264 ;
    dct:isReferencedBy F2021L00334: ;
    rdfs:comment "8 2  Person who must give notice of intention to export - Abrievated Graph Key: I266"@en-AU ;
    skos:definition "8 2  Person who must give notice of intention to export"@en-AU ;
    skos:narrower F2021L00334:264 ;
    skos:prefLabel "Item I266"@en-AU ;
    dcat:accessURL <https://www.legislation.gov.au/F2021L00334/2023-08-04/2023-08-04/text/original/epub/OEBPS/document_1/document_1.html#_Toc143507913> ;
    dcat:landingPage "https://www.legislation.gov.au/F2021L00334/2023-08-04/2023-08-04/text/original/epub/OEBPS/document_1/document_1.html#_Toc143507913"^^xsd:anyURI ;
    dcat:theme legcons:Item .

F2021L00334:267 a legcons:Item,
        owl:Class,
        dcat:Resource ;
    rdfs:label "Item - I267 8 3  Person to whom notice of intention to export must be given"@en-AU ;
    dct:isPartOf F2021L00334:264 ;
    dct:isReferencedBy F2021L00334: ;
    rdfs:comment "8 3  Person to whom notice of intention to export must be given - Abrievated Graph Key: I267"@en-AU ;
    skos:definition "8 3  Person to whom notice of intention to export must be given"@en-AU ;
    skos:narrower F2021L00334:264 ;
    skos:prefLabel "Item I267"@en-AU ;
    dcat:accessURL <https://www.legislation.gov.au/F2021L00334/2023-08-04/2023-08-04/text/original/epub/OEBPS/document_1/document_1.html#_Toc143507914> ;
    dcat:landingPage "https://www.legislation.gov.au/F2021L00334/2023-08-04/2023-08-04/text/original/epub/OEBPS/document_1/document_1.html#_Toc143507914"^^xsd:anyURI ;
    dcat:theme legcons:Item .

F2021L00334:268 a legcons:Item,
        owl:Class,
        dcat:Resource ;
    rdfs:label "Item - I268 8 4  When notice of intention to export must be given"@en-AU ;
    dct:isPartOf F2021L00334:264 ;
    dct:isReferencedBy F2021L00334: ;
    rdfs:comment "8 4  When notice of intention to export must be given - Abrievated Graph Key: I268"@en-AU ;
    skos:definition "8 4  When notice of intention to export must be given"@en-AU ;
    skos:narrower F2021L00334:264 ;
    skos:prefLabel "Item I268"@en-AU ;
    dcat:accessURL <https://www.legislation.gov.au/F2021L00334/2023-08-04/2023-08-04/text/original/epub/OEBPS/document_1/document_1.html#_Toc143507915> ;
    dcat:landingPage "https://www.legislation.gov.au/F2021L00334/2023-08-04/2023-08-04/text/original/epub/OEBPS/document_1/document_1.html#_Toc143507915"^^xsd:anyURI ;
    dcat:theme legcons:Item .

F2021L00334:27 a legcons:Item,
        owl:Class,
        dcat:Resource ;
    rdfs:label "Item - I27 2 9  Variation of conditions of exemptionmatters to which Secretary must have regard"@en-AU ;
    dct:isPartOf F2021L00334:22 ;
    dct:isReferencedBy F2021L00334: ;
    rdfs:comment "2 9  Variation of conditions of exemptionmatters to which Secretary must have regard - Abrievated Graph Key: I27"@en-AU ;
    skos:definition "2 9  Variation of conditions of exemptionmatters to which Secretary must have regard"@en-AU ;
    skos:narrower F2021L00334:22 ;
    skos:prefLabel "Item I27"@en-AU ;
    dcat:accessURL <https://www.legislation.gov.au/F2021L00334/2023-08-04/2023-08-04/text/original/epub/OEBPS/document_1/document_1.html#_Toc143507674> ;
    dcat:landingPage "https://www.legislation.gov.au/F2021L00334/2023-08-04/2023-08-04/text/original/epub/OEBPS/document_1/document_1.html#_Toc143507674"^^xsd:anyURI ;
    dcat:theme legcons:Item .

F2021L00334:270 a legcons:Item,
        owl:Class,
        dcat:Resource ;
    rdfs:label "Item - I270 8 5  Purpose of this Part"@en-AU ;
    dct:isPartOf F2021L00334:269 ;
    dct:isReferencedBy F2021L00334: ;
    rdfs:comment "8 5  Purpose of this Part - Abrievated Graph Key: I270"@en-AU ;
    skos:definition "8 5  Purpose of this Part"@en-AU ;
    skos:narrower F2021L00334:269 ;
    skos:prefLabel "Item I270"@en-AU ;
    dcat:accessURL <https://www.legislation.gov.au/F2021L00334/2023-08-04/2023-08-04/text/original/epub/OEBPS/document_1/document_1.html#_Toc143507917> ;
    dcat:landingPage "https://www.legislation.gov.au/F2021L00334/2023-08-04/2023-08-04/text/original/epub/OEBPS/document_1/document_1.html#_Toc143507917"^^xsd:anyURI ;
    dcat:theme legcons:Item .

F2021L00334:271 a legcons:Item,
        owl:Class,
        dcat:Resource ;
    rdfs:label "Item - I271 8 6  General requirements for trade descriptions"@en-AU ;
    dct:isPartOf F2021L00334:269 ;
    dct:isReferencedBy F2021L00334: ;
    rdfs:comment "8 6  General requirements for trade descriptions - Abrievated Graph Key: I271"@en-AU ;
    skos:definition "8 6  General requirements for trade descriptions"@en-AU ;
    skos:narrower F2021L00334:269 ;
    skos:prefLabel "Item I271"@en-AU ;
    dcat:accessURL <https://www.legislation.gov.au/F2021L00334/2023-08-04/2023-08-04/text/original/epub/OEBPS/document_1/document_1.html#_Toc143507918> ;
    dcat:landingPage "https://www.legislation.gov.au/F2021L00334/2023-08-04/2023-08-04/text/original/epub/OEBPS/document_1/document_1.html#_Toc143507918"^^xsd:anyURI ;
    dcat:theme legcons:Item .

F2021L00334:272 a legcons:Item,
        owl:Class,
        dcat:Resource ;
    rdfs:label "Item - I272 8 7  Trade descriptions in language other than English"@en-AU ;
    dct:isPartOf F2021L00334:269 ;
    dct:isReferencedBy F2021L00334: ;
    rdfs:comment "8 7  Trade descriptions in language other than English - Abrievated Graph Key: I272"@en-AU ;
    skos:definition "8 7  Trade descriptions in language other than English"@en-AU ;
    skos:narrower F2021L00334:269 ;
    skos:prefLabel "Item I272"@en-AU ;
    dcat:accessURL <https://www.legislation.gov.au/F2021L00334/2023-08-04/2023-08-04/text/original/epub/OEBPS/document_1/document_1.html#_Toc143507919> ;
    dcat:landingPage "https://www.legislation.gov.au/F2021L00334/2023-08-04/2023-08-04/text/original/epub/OEBPS/document_1/document_1.html#_Toc143507919"^^xsd:anyURI ;
    dcat:theme legcons:Item .

F2021L00334:275 a legcons:Item,
        owl:Class,
        dcat:Resource ;
    rdfs:label "Item - I275 8 8  Purpose of this Division"@en-AU ;
    dct:isPartOf F2021L00334:274 ;
    dct:isReferencedBy F2021L00334: ;
    rdfs:comment "8 8  Purpose of this Division - Abrievated Graph Key: I275"@en-AU ;
    skos:definition "8 8  Purpose of this Division"@en-AU ;
    skos:narrower F2021L00334:274 ;
    skos:prefLabel "Item I275"@en-AU ;
    dcat:accessURL <https://www.legislation.gov.au/F2021L00334/2023-08-04/2023-08-04/text/original/epub/OEBPS/document_1/document_1.html#_Toc143507922> ;
    dcat:landingPage "https://www.legislation.gov.au/F2021L00334/2023-08-04/2023-08-04/text/original/epub/OEBPS/document_1/document_1.html#_Toc143507922"^^xsd:anyURI ;
    dcat:theme legcons:Item .

F2021L00334:276 a legcons:Item,
        owl:Class,
        dcat:Resource ;
    rdfs:label "Item - I276 8 9  Tolerances for dimensions of official marks"@en-AU ;
    dct:isPartOf F2021L00334:274 ;
    dct:isReferencedBy F2021L00334: ;
    rdfs:comment "8 9  Tolerances for dimensions of official marks - Abrievated Graph Key: I276"@en-AU ;
    skos:definition "8 9  Tolerances for dimensions of official marks"@en-AU ;
    skos:narrower F2021L00334:274 ;
    skos:prefLabel "Item I276"@en-AU ;
    dcat:accessURL <https://www.legislation.gov.au/F2021L00334/2023-08-04/2023-08-04/text/original/epub/OEBPS/document_1/document_1.html#_Toc143507923> ;
    dcat:landingPage "https://www.legislation.gov.au/F2021L00334/2023-08-04/2023-08-04/text/original/epub/OEBPS/document_1/document_1.html#_Toc143507923"^^xsd:anyURI ;
    dcat:theme legcons:Item .

F2021L00334:277 a legcons:Item,
        owl:Class,
        dcat:Resource ;
    rdfs:label "Item - I277 8 10  Official markAustralia Inspected"@en-AU ;
    dct:isPartOf F2021L00334:274 ;
    dct:isReferencedBy F2021L00334: ;
    rdfs:comment "8 10  Official markAustralia Inspected - Abrievated Graph Key: I277"@en-AU ;
    skos:definition "8 10  Official markAustralia Inspected"@en-AU ;
    skos:narrower F2021L00334:274 ;
    skos:prefLabel "Item I277"@en-AU ;
    dcat:accessURL <https://www.legislation.gov.au/F2021L00334/2023-08-04/2023-08-04/text/original/epub/OEBPS/document_1/document_1.html#_Toc143507924> ;
    dcat:landingPage "https://www.legislation.gov.au/F2021L00334/2023-08-04/2023-08-04/text/original/epub/OEBPS/document_1/document_1.html#_Toc143507924"^^xsd:anyURI ;
    dcat:theme legcons:Item .

F2021L00334:278 a legcons:Item,
        owl:Class,
        dcat:Resource ;
    rdfs:label "Item - I278 8 11  Official markAustralia Inspected lamb"@en-AU ;
    dct:isPartOf F2021L00334:274 ;
    dct:isReferencedBy F2021L00334: ;
    rdfs:comment "8 11  Official markAustralia Inspected lamb - Abrievated Graph Key: I278"@en-AU ;
    skos:definition "8 11  Official markAustralia Inspected lamb"@en-AU ;
    skos:narrower F2021L00334:274 ;
    skos:prefLabel "Item I278"@en-AU ;
    dcat:accessURL <https://www.legislation.gov.au/F2021L00334/2023-08-04/2023-08-04/text/original/epub/OEBPS/document_1/document_1.html#_Toc143507925> ;
    dcat:landingPage "https://www.legislation.gov.au/F2021L00334/2023-08-04/2023-08-04/text/original/epub/OEBPS/document_1/document_1.html#_Toc143507925"^^xsd:anyURI ;
    dcat:theme legcons:Item .

F2021L00334:279 a legcons:Item,
        owl:Class,
        dcat:Resource ;
    rdfs:label "Item - I279 8 12  Official markHalal meat"@en-AU ;
    dct:isPartOf F2021L00334:274 ;
    dct:isReferencedBy F2021L00334: ;
    rdfs:comment "8 12  Official markHalal meat - Abrievated Graph Key: I279"@en-AU ;
    skos:definition "8 12  Official markHalal meat"@en-AU ;
    skos:narrower F2021L00334:274 ;
    skos:prefLabel "Item I279"@en-AU ;
    dcat:accessURL <https://www.legislation.gov.au/F2021L00334/2023-08-04/2023-08-04/text/original/epub/OEBPS/document_1/document_1.html#_Toc143507926> ;
    dcat:landingPage "https://www.legislation.gov.au/F2021L00334/2023-08-04/2023-08-04/text/original/epub/OEBPS/document_1/document_1.html#_Toc143507926"^^xsd:anyURI ;
    dcat:theme legcons:Item .

F2021L00334:28 a legcons:Item,
        owl:Class,
        dcat:Resource ;
    rdfs:label "Item - I28 2 10  Revocation of exemptionmatters to which Secretary must have regard"@en-AU ;
    dct:isPartOf F2021L00334:22 ;
    dct:isReferencedBy F2021L00334: ;
    rdfs:comment "2 10  Revocation of exemptionmatters to which Secretary must have regard - Abrievated Graph Key: I28"@en-AU ;
    skos:definition "2 10  Revocation of exemptionmatters to which Secretary must have regard"@en-AU ;
    skos:narrower F2021L00334:22 ;
    skos:prefLabel "Item I28"@en-AU ;
    dcat:accessURL <https://www.legislation.gov.au/F2021L00334/2023-08-04/2023-08-04/text/original/epub/OEBPS/document_1/document_1.html#_Toc143507675> ;
    dcat:landingPage "https://www.legislation.gov.au/F2021L00334/2023-08-04/2023-08-04/text/original/epub/OEBPS/document_1/document_1.html#_Toc143507675"^^xsd:anyURI ;
    dcat:theme legcons:Item .

F2021L00334:280 a legcons:Item,
        owl:Class,
        dcat:Resource ;
    rdfs:label "Item - I280 8 13  Official markforeign country identification"@en-AU ;
    dct:isPartOf F2021L00334:274 ;
    dct:isReferencedBy F2021L00334: ;
    rdfs:comment "8 13  Official markforeign country identification - Abrievated Graph Key: I280"@en-AU ;
    skos:definition "8 13  Official markforeign country identification"@en-AU ;
    skos:narrower F2021L00334:274 ;
    skos:prefLabel "Item I280"@en-AU ;
    dcat:accessURL <https://www.legislation.gov.au/F2021L00334/2023-08-04/2023-08-04/text/original/epub/OEBPS/document_1/document_1.html#_Toc143507927> ;
    dcat:landingPage "https://www.legislation.gov.au/F2021L00334/2023-08-04/2023-08-04/text/original/epub/OEBPS/document_1/document_1.html#_Toc143507927"^^xsd:anyURI ;
    dcat:theme legcons:Item .

F2021L00334:281 a legcons:Item,
        owl:Class,
        dcat:Resource ;
    rdfs:label "Item - I281 8 14  Official marktamper indicative metal strap seal"@en-AU ;
    dct:isPartOf F2021L00334:274 ;
    dct:isReferencedBy F2021L00334: ;
    rdfs:comment "8 14  Official marktamper indicative metal strap seal - Abrievated Graph Key: I281"@en-AU ;
    skos:definition "8 14  Official marktamper indicative metal strap seal"@en-AU ;
    skos:narrower F2021L00334:274 ;
    skos:prefLabel "Item I281"@en-AU ;
    dcat:accessURL <https://www.legislation.gov.au/F2021L00334/2023-08-04/2023-08-04/text/original/epub/OEBPS/document_1/document_1.html#_Toc143507928> ;
    dcat:landingPage "https://www.legislation.gov.au/F2021L00334/2023-08-04/2023-08-04/text/original/epub/OEBPS/document_1/document_1.html#_Toc143507928"^^xsd:anyURI ;
    dcat:theme legcons:Item .

F2021L00334:282 a legcons:Item,
        owl:Class,
        dcat:Resource ;
    rdfs:label "Item - I282 8 15  Official markbolt seal"@en-AU ;
    dct:isPartOf F2021L00334:274 ;
    dct:isReferencedBy F2021L00334: ;
    rdfs:comment "8 15  Official markbolt seal - Abrievated Graph Key: I282"@en-AU ;
    skos:definition "8 15  Official markbolt seal"@en-AU ;
    skos:narrower F2021L00334:274 ;
    skos:prefLabel "Item I282"@en-AU ;
    dcat:accessURL <https://www.legislation.gov.au/F2021L00334/2023-08-04/2023-08-04/text/original/epub/OEBPS/document_1/document_1.html#_Toc143507929> ;
    dcat:landingPage "https://www.legislation.gov.au/F2021L00334/2023-08-04/2023-08-04/text/original/epub/OEBPS/document_1/document_1.html#_Toc143507929"^^xsd:anyURI ;
    dcat:theme legcons:Item .

F2021L00334:283 a legcons:Item,
        owl:Class,
        dcat:Resource ;
    rdfs:label "Item - I283 8 16  Official markAustralia Approved"@en-AU ;
    dct:isPartOf F2021L00334:274 ;
    dct:isReferencedBy F2021L00334: ;
    rdfs:comment "8 16  Official markAustralia Approved - Abrievated Graph Key: I283"@en-AU ;
    skos:definition "8 16  Official markAustralia Approved"@en-AU ;
    skos:narrower F2021L00334:274 ;
    skos:prefLabel "Item I283"@en-AU ;
    dcat:accessURL <https://www.legislation.gov.au/F2021L00334/2023-08-04/2023-08-04/text/original/epub/OEBPS/document_1/document_1.html#_Toc143507930> ;
    dcat:landingPage "https://www.legislation.gov.au/F2021L00334/2023-08-04/2023-08-04/text/original/epub/OEBPS/document_1/document_1.html#_Toc143507930"^^xsd:anyURI ;
    dcat:theme legcons:Item .

F2021L00334:284 a legcons:Item,
        owl:Class,
        dcat:Resource ;
    rdfs:label "Item - I284 8 17  Official markAustralia Approved lamb"@en-AU ;
    dct:isPartOf F2021L00334:274 ;
    dct:isReferencedBy F2021L00334: ;
    rdfs:comment "8 17  Official markAustralia Approved lamb - Abrievated Graph Key: I284"@en-AU ;
    skos:definition "8 17  Official markAustralia Approved lamb"@en-AU ;
    skos:narrower F2021L00334:274 ;
    skos:prefLabel "Item I284"@en-AU ;
    dcat:accessURL <https://www.legislation.gov.au/F2021L00334/2023-08-04/2023-08-04/text/original/epub/OEBPS/document_1/document_1.html#_Toc143507931> ;
    dcat:landingPage "https://www.legislation.gov.au/F2021L00334/2023-08-04/2023-08-04/text/original/epub/OEBPS/document_1/document_1.html#_Toc143507931"^^xsd:anyURI ;
    dcat:theme legcons:Item .

F2021L00334:285 a legcons:Item,
        owl:Class,
        dcat:Resource ;
    rdfs:label "Item - I285 8 18  Official markEuropean Union"@en-AU ;
    dct:isPartOf F2021L00334:274 ;
    dct:isReferencedBy F2021L00334: ;
    rdfs:comment "8 18  Official markEuropean Union - Abrievated Graph Key: I285"@en-AU ;
    skos:definition "8 18  Official markEuropean Union"@en-AU ;
    skos:narrower F2021L00334:274 ;
    skos:prefLabel "Item I285"@en-AU ;
    dcat:accessURL <https://www.legislation.gov.au/F2021L00334/2023-08-04/2023-08-04/text/original/epub/OEBPS/document_1/document_1.html#_Toc143507932> ;
    dcat:landingPage "https://www.legislation.gov.au/F2021L00334/2023-08-04/2023-08-04/text/original/epub/OEBPS/document_1/document_1.html#_Toc143507932"^^xsd:anyURI ;
    dcat:theme legcons:Item .

F2021L00334:286 a legcons:Item,
        owl:Class,
        dcat:Resource ;
    rdfs:label "Item - I286 8 19  Official markcarton seal"@en-AU ;
    dct:isPartOf F2021L00334:274 ;
    dct:isReferencedBy F2021L00334: ;
    rdfs:comment "8 19  Official markcarton seal - Abrievated Graph Key: I286"@en-AU ;
    skos:definition "8 19  Official markcarton seal"@en-AU ;
    skos:narrower F2021L00334:274 ;
    skos:prefLabel "Item I286"@en-AU ;
    dcat:accessURL <https://www.legislation.gov.au/F2021L00334/2023-08-04/2023-08-04/text/original/epub/OEBPS/document_1/document_1.html#_Toc143507933> ;
    dcat:landingPage "https://www.legislation.gov.au/F2021L00334/2023-08-04/2023-08-04/text/original/epub/OEBPS/document_1/document_1.html#_Toc143507933"^^xsd:anyURI ;
    dcat:theme legcons:Item .

F2021L00334:287 a legcons:Item,
        owl:Class,
        dcat:Resource ;
    rdfs:label "Item - I287 8 20  Official markmeat or meat products opened for assessment and resealed"@en-AU ;
    dct:isPartOf F2021L00334:274 ;
    dct:isReferencedBy F2021L00334: ;
    rdfs:comment "8 20  Official markmeat or meat products opened for assessment and resealed - Abrievated Graph Key: I287"@en-AU ;
    skos:definition "8 20  Official markmeat or meat products opened for assessment and resealed"@en-AU ;
    skos:narrower F2021L00334:274 ;
    skos:prefLabel "Item I287"@en-AU ;
    dcat:accessURL <https://www.legislation.gov.au/F2021L00334/2023-08-04/2023-08-04/text/original/epub/OEBPS/document_1/document_1.html#_Toc143507934> ;
    dcat:landingPage "https://www.legislation.gov.au/F2021L00334/2023-08-04/2023-08-04/text/original/epub/OEBPS/document_1/document_1.html#_Toc143507934"^^xsd:anyURI ;
    dcat:theme legcons:Item .

F2021L00334:288 a legcons:Item,
        owl:Class,
        dcat:Resource ;
    rdfs:label "Item - I288 8 21  Official markAustralian Government"@en-AU ;
    dct:isPartOf F2021L00334:274 ;
    dct:isReferencedBy F2021L00334: ;
    rdfs:comment "8 21  Official markAustralian Government - Abrievated Graph Key: I288"@en-AU ;
    skos:definition "8 21  Official markAustralian Government"@en-AU ;
    skos:narrower F2021L00334:274 ;
    skos:prefLabel "Item I288"@en-AU ;
    dcat:accessURL <https://www.legislation.gov.au/F2021L00334/2023-08-04/2023-08-04/text/original/epub/OEBPS/document_1/document_1.html#_Toc143507935> ;
    dcat:landingPage "https://www.legislation.gov.au/F2021L00334/2023-08-04/2023-08-04/text/original/epub/OEBPS/document_1/document_1.html#_Toc143507935"^^xsd:anyURI ;
    dcat:theme legcons:Item .

F2021L00334:290 a legcons:Item,
        owl:Class,
        dcat:Resource ;
    rdfs:label "Item - I290 8 22  Purpose and application of this Division"@en-AU ;
    dct:isPartOf F2021L00334:289 ;
    dct:isReferencedBy F2021L00334: ;
    rdfs:comment "8 22  Purpose and application of this Division - Abrievated Graph Key: I290"@en-AU ;
    skos:definition "8 22  Purpose and application of this Division"@en-AU ;
    skos:narrower F2021L00334:289 ;
    skos:prefLabel "Item I290"@en-AU ;
    dcat:accessURL <https://www.legislation.gov.au/F2021L00334/2023-08-04/2023-08-04/text/original/epub/OEBPS/document_1/document_1.html#_Toc143507937> ;
    dcat:landingPage "https://www.legislation.gov.au/F2021L00334/2023-08-04/2023-08-04/text/original/epub/OEBPS/document_1/document_1.html#_Toc143507937"^^xsd:anyURI ;
    dcat:theme legcons:Item .

F2021L00334:291 a legcons:Item,
        owl:Class,
        dcat:Resource ;
    rdfs:label "Item - I291 8 23  Interpretation"@en-AU ;
    dct:isPartOf F2021L00334:289 ;
    dct:isReferencedBy F2021L00334: ;
    rdfs:comment "8 23  Interpretation - Abrievated Graph Key: I291"@en-AU ;
    skos:definition "8 23  Interpretation"@en-AU ;
    skos:narrower F2021L00334:289 ;
    skos:prefLabel "Item I291"@en-AU ;
    dcat:accessURL <https://www.legislation.gov.au/F2021L00334/2023-08-04/2023-08-04/text/original/epub/OEBPS/document_1/document_1.html#_Toc143507938> ;
    dcat:landingPage "https://www.legislation.gov.au/F2021L00334/2023-08-04/2023-08-04/text/original/epub/OEBPS/document_1/document_1.html#_Toc143507938"^^xsd:anyURI ;
    dcat:theme legcons:Item .

F2021L00334:292 a legcons:Item,
        owl:Class,
        dcat:Resource ;
    rdfs:label "Item - I292 8 24  Persons who may manufacture or supply official marks for meat or meat products"@en-AU ;
    dct:isPartOf F2021L00334:289 ;
    dct:isReferencedBy F2021L00334: ;
    rdfs:comment "8 24  Persons who may manufacture or supply official marks for meat or meat products - Abrievated Graph Key: I292"@en-AU ;
    skos:definition "8 24  Persons who may manufacture or supply official marks for meat or meat products"@en-AU ;
    skos:narrower F2021L00334:289 ;
    skos:prefLabel "Item I292"@en-AU ;
    dcat:accessURL <https://www.legislation.gov.au/F2021L00334/2023-08-04/2023-08-04/text/original/epub/OEBPS/document_1/document_1.html#_Toc143507939> ;
    dcat:landingPage "https://www.legislation.gov.au/F2021L00334/2023-08-04/2023-08-04/text/original/epub/OEBPS/document_1/document_1.html#_Toc143507939"^^xsd:anyURI ;
    dcat:theme legcons:Item .

F2021L00334:293 a legcons:Item,
        owl:Class,
        dcat:Resource ;
    rdfs:label "Item - I293 8 25  Persons who may possess official marks that have not been applied to meat or meat products"@en-AU ;
    dct:isPartOf F2021L00334:289 ;
    dct:isReferencedBy F2021L00334: ;
    rdfs:comment "8 25  Persons who may possess official marks that have not been applied to meat or meat products - Abrievated Graph Key: I293"@en-AU ;
    skos:definition "8 25  Persons who may possess official marks that have not been applied to meat or meat products"@en-AU ;
    skos:narrower F2021L00334:289 ;
    skos:prefLabel "Item I293"@en-AU ;
    dcat:accessURL <https://www.legislation.gov.au/F2021L00334/2023-08-04/2023-08-04/text/original/epub/OEBPS/document_1/document_1.html#_Toc143507940> ;
    dcat:landingPage "https://www.legislation.gov.au/F2021L00334/2023-08-04/2023-08-04/text/original/epub/OEBPS/document_1/document_1.html#_Toc143507940"^^xsd:anyURI ;
    dcat:theme legcons:Item .

F2021L00334:294 a legcons:Item,
        owl:Class,
        dcat:Resource ;
    rdfs:label "Item - I294 8 26  Persons who may apply official marks to meat or meat products etc"@en-AU ;
    dct:isPartOf F2021L00334:289 ;
    dct:isReferencedBy F2021L00334: ;
    rdfs:comment "8 26  Persons who may apply official marks to meat or meat products etc - Abrievated Graph Key: I294"@en-AU ;
    skos:definition "8 26  Persons who may apply official marks to meat or meat products etc"@en-AU ;
    skos:narrower F2021L00334:289 ;
    skos:prefLabel "Item I294"@en-AU ;
    dcat:accessURL <https://www.legislation.gov.au/F2021L00334/2023-08-04/2023-08-04/text/original/epub/OEBPS/document_1/document_1.html#_Toc143507941> ;
    dcat:landingPage "https://www.legislation.gov.au/F2021L00334/2023-08-04/2023-08-04/text/original/epub/OEBPS/document_1/document_1.html#_Toc143507941"^^xsd:anyURI ;
    dcat:theme legcons:Item .

F2021L00334:295 a legcons:Item,
        owl:Class,
        dcat:Resource ;
    rdfs:label "Item - I295 8 27  Circumstances in which official mark must not be applied to meat or meat products"@en-AU ;
    dct:isPartOf F2021L00334:289 ;
    dct:isReferencedBy F2021L00334: ;
    rdfs:comment "8 27  Circumstances in which official mark must not be applied to meat or meat products - Abrievated Graph Key: I295"@en-AU ;
    skos:definition "8 27  Circumstances in which official mark must not be applied to meat or meat products"@en-AU ;
    skos:narrower F2021L00334:289 ;
    skos:prefLabel "Item I295"@en-AU ;
    dcat:accessURL <https://www.legislation.gov.au/F2021L00334/2023-08-04/2023-08-04/text/original/epub/OEBPS/document_1/document_1.html#_Toc143507942> ;
    dcat:landingPage "https://www.legislation.gov.au/F2021L00334/2023-08-04/2023-08-04/text/original/epub/OEBPS/document_1/document_1.html#_Toc143507942"^^xsd:anyURI ;
    dcat:theme legcons:Item .

F2021L00334:296 a legcons:Item,
        owl:Class,
        dcat:Resource ;
    rdfs:label "Item - I296 8 28  Alteration of and interference with official marks"@en-AU ;
    dct:isPartOf F2021L00334:289 ;
    dct:isReferencedBy F2021L00334: ;
    rdfs:comment "8 28  Alteration of and interference with official marks - Abrievated Graph Key: I296"@en-AU ;
    skos:definition "8 28  Alteration of and interference with official marks"@en-AU ;
    skos:narrower F2021L00334:289 ;
    skos:prefLabel "Item I296"@en-AU ;
    dcat:accessURL <https://www.legislation.gov.au/F2021L00334/2023-08-04/2023-08-04/text/original/epub/OEBPS/document_1/document_1.html#_Toc143507943> ;
    dcat:landingPage "https://www.legislation.gov.au/F2021L00334/2023-08-04/2023-08-04/text/original/epub/OEBPS/document_1/document_1.html#_Toc143507943"^^xsd:anyURI ;
    dcat:theme legcons:Item .

F2021L00334:297 a legcons:Item,
        owl:Class,
        dcat:Resource ;
    rdfs:label "Item - I297 8 29  Official marks must be legible and securely attached"@en-AU ;
    dct:isPartOf F2021L00334:289 ;
    dct:isReferencedBy F2021L00334: ;
    rdfs:comment "8 29  Official marks must be legible and securely attached - Abrievated Graph Key: I297"@en-AU ;
    skos:definition "8 29  Official marks must be legible and securely attached"@en-AU ;
    skos:narrower F2021L00334:289 ;
    skos:prefLabel "Item I297"@en-AU ;
    dcat:accessURL <https://www.legislation.gov.au/F2021L00334/2023-08-04/2023-08-04/text/original/epub/OEBPS/document_1/document_1.html#_Toc143507944> ;
    dcat:landingPage "https://www.legislation.gov.au/F2021L00334/2023-08-04/2023-08-04/text/original/epub/OEBPS/document_1/document_1.html#_Toc143507944"^^xsd:anyURI ;
    dcat:theme legcons:Item .

F2021L00334:298 a legcons:Item,
        owl:Class,
        dcat:Resource ;
    rdfs:label "Item - I298 8 30  Security of official marks"@en-AU ;
    dct:isPartOf F2021L00334:289 ;
    dct:isReferencedBy F2021L00334: ;
    rdfs:comment "8 30  Security of official marks - Abrievated Graph Key: I298"@en-AU ;
    skos:definition "8 30  Security of official marks"@en-AU ;
    skos:narrower F2021L00334:289 ;
    skos:prefLabel "Item I298"@en-AU ;
    dcat:accessURL <https://www.legislation.gov.au/F2021L00334/2023-08-04/2023-08-04/text/original/epub/OEBPS/document_1/document_1.html#_Toc143507945> ;
    dcat:landingPage "https://www.legislation.gov.au/F2021L00334/2023-08-04/2023-08-04/text/original/epub/OEBPS/document_1/document_1.html#_Toc143507945"^^xsd:anyURI ;
    dcat:theme legcons:Item .

F2021L00334:299 a legcons:Item,
        owl:Class,
        dcat:Resource ;
    rdfs:label "Item - I299 8 31  Removal or defacement of official marks"@en-AU ;
    dct:isPartOf F2021L00334:289 ;
    dct:isReferencedBy F2021L00334: ;
    rdfs:comment "8 31  Removal or defacement of official marks - Abrievated Graph Key: I299"@en-AU ;
    skos:definition "8 31  Removal or defacement of official marks"@en-AU ;
    skos:narrower F2021L00334:289 ;
    skos:prefLabel "Item I299"@en-AU ;
    dcat:accessURL <https://www.legislation.gov.au/F2021L00334/2023-08-04/2023-08-04/text/original/epub/OEBPS/document_1/document_1.html#_Toc143507946> ;
    dcat:landingPage "https://www.legislation.gov.au/F2021L00334/2023-08-04/2023-08-04/text/original/epub/OEBPS/document_1/document_1.html#_Toc143507946"^^xsd:anyURI ;
    dcat:theme legcons:Item .

F2021L00334:3 a legcons:Item,
        owl:Class,
        dcat:Resource ;
    rdfs:label "Item - I3 1 1  Name"@en-AU ;
    dct:isPartOf F2021L00334:1 ;
    dct:isReferencedBy F2021L00334: ;
    rdfs:comment "1 1  Name - Abrievated Graph Key: I3"@en-AU ;
    skos:definition "1 1  Name"@en-AU ;
    skos:narrower F2021L00334:1 ;
    skos:prefLabel "Item I3"@en-AU ;
    dcat:accessURL <https://www.legislation.gov.au/F2021L00334/2023-08-04/2023-08-04/text/original/epub/OEBPS/document_1/document_1.html#_Toc143507650> ;
    dcat:landingPage "https://www.legislation.gov.au/F2021L00334/2023-08-04/2023-08-04/text/original/epub/OEBPS/document_1/document_1.html#_Toc143507650"^^xsd:anyURI ;
    dcat:theme legcons:Item .

F2021L00334:30 a legcons:Item,
        owl:Class,
        dcat:Resource ;
    rdfs:label "Item - I30 2 11  When government certificate may be issued in relation to meat or meat products"@en-AU ;
    dct:isPartOf F2021L00334:29 ;
    dct:isReferencedBy F2021L00334: ;
    rdfs:comment "2 11  When government certificate may be issued in relation to meat or meat products - Abrievated Graph Key: I30"@en-AU ;
    skos:definition "2 11  When government certificate may be issued in relation to meat or meat products"@en-AU ;
    skos:narrower F2021L00334:29 ;
    skos:prefLabel "Item I30"@en-AU ;
    dcat:accessURL <https://www.legislation.gov.au/F2021L00334/2023-08-04/2023-08-04/text/original/epub/OEBPS/document_1/document_1.html#_Toc143507677> ;
    dcat:landingPage "https://www.legislation.gov.au/F2021L00334/2023-08-04/2023-08-04/text/original/epub/OEBPS/document_1/document_1.html#_Toc143507677"^^xsd:anyURI ;
    dcat:theme legcons:Item .

F2021L00334:300 a legcons:Item,
        owl:Class,
        dcat:Resource ;
    rdfs:label "Item - I300 8 32  Records of official marks manufactured or supplied"@en-AU ;
    dct:isPartOf F2021L00334:289 ;
    dct:isReferencedBy F2021L00334: ;
    rdfs:comment "8 32  Records of official marks manufactured or supplied - Abrievated Graph Key: I300"@en-AU ;
    skos:definition "8 32  Records of official marks manufactured or supplied"@en-AU ;
    skos:narrower F2021L00334:289 ;
    skos:prefLabel "Item I300"@en-AU ;
    dcat:accessURL <https://www.legislation.gov.au/F2021L00334/2023-08-04/2023-08-04/text/original/epub/OEBPS/document_1/document_1.html#_Toc143507947> ;
    dcat:landingPage "https://www.legislation.gov.au/F2021L00334/2023-08-04/2023-08-04/text/original/epub/OEBPS/document_1/document_1.html#_Toc143507947"^^xsd:anyURI ;
    dcat:theme legcons:Item .

F2021L00334:301 a legcons:Item,
        owl:Class,
        dcat:Resource ;
    rdfs:label "Item - I301 8 33  Records of official marks received applied removed defaced destroyed or returned"@en-AU ;
    dct:isPartOf F2021L00334:289 ;
    dct:isReferencedBy F2021L00334: ;
    rdfs:comment "8 33  Records of official marks received applied removed defaced destroyed or returned - Abrievated Graph Key: I301"@en-AU ;
    skos:definition "8 33  Records of official marks received applied removed defaced destroyed or returned"@en-AU ;
    skos:narrower F2021L00334:289 ;
    skos:prefLabel "Item I301"@en-AU ;
    dcat:accessURL <https://www.legislation.gov.au/F2021L00334/2023-08-04/2023-08-04/text/original/epub/OEBPS/document_1/document_1.html#_Toc143507948> ;
    dcat:landingPage "https://www.legislation.gov.au/F2021L00334/2023-08-04/2023-08-04/text/original/epub/OEBPS/document_1/document_1.html#_Toc143507948"^^xsd:anyURI ;
    dcat:theme legcons:Item .

F2021L00334:303 a legcons:Item,
        owl:Class,
        dcat:Resource ;
    rdfs:label "Item - I303 8 34  Purpose of this Division"@en-AU ;
    dct:isPartOf F2021L00334:302 ;
    dct:isReferencedBy F2021L00334: ;
    rdfs:comment "8 34  Purpose of this Division - Abrievated Graph Key: I303"@en-AU ;
    skos:definition "8 34  Purpose of this Division"@en-AU ;
    skos:narrower F2021L00334:302 ;
    skos:prefLabel "Item I303"@en-AU ;
    dcat:accessURL <https://www.legislation.gov.au/F2021L00334/2023-08-04/2023-08-04/text/original/epub/OEBPS/document_1/document_1.html#_Toc143507950> ;
    dcat:landingPage "https://www.legislation.gov.au/F2021L00334/2023-08-04/2023-08-04/text/original/epub/OEBPS/document_1/document_1.html#_Toc143507950"^^xsd:anyURI ;
    dcat:theme legcons:Item .

F2021L00334:304 a legcons:Item,
        owl:Class,
        dcat:Resource ;
    rdfs:label "Item - I304 8 35  Circumstances in which a mark resembles an official mark"@en-AU ;
    dct:isPartOf F2021L00334:302 ;
    dct:isReferencedBy F2021L00334: ;
    rdfs:comment "8 35  Circumstances in which a mark resembles an official mark - Abrievated Graph Key: I304"@en-AU ;
    skos:definition "8 35  Circumstances in which a mark resembles an official mark"@en-AU ;
    skos:narrower F2021L00334:302 ;
    skos:prefLabel "Item I304"@en-AU ;
    dcat:accessURL <https://www.legislation.gov.au/F2021L00334/2023-08-04/2023-08-04/text/original/epub/OEBPS/document_1/document_1.html#_Toc143507951> ;
    dcat:landingPage "https://www.legislation.gov.au/F2021L00334/2023-08-04/2023-08-04/text/original/epub/OEBPS/document_1/document_1.html#_Toc143507951"^^xsd:anyURI ;
    dcat:theme legcons:Item .

F2021L00334:305 a legcons:Item,
        owl:Class,
        dcat:Resource ;
    rdfs:label "Item - I305 8 36  Persons who may apply a resemblance"@en-AU ;
    dct:isPartOf F2021L00334:302 ;
    dct:isReferencedBy F2021L00334: ;
    rdfs:comment "8 36  Persons who may apply a resemblance - Abrievated Graph Key: I305"@en-AU ;
    skos:definition "8 36  Persons who may apply a resemblance"@en-AU ;
    skos:narrower F2021L00334:302 ;
    skos:prefLabel "Item I305"@en-AU ;
    dcat:accessURL <https://www.legislation.gov.au/F2021L00334/2023-08-04/2023-08-04/text/original/epub/OEBPS/document_1/document_1.html#_Toc143507952> ;
    dcat:landingPage "https://www.legislation.gov.au/F2021L00334/2023-08-04/2023-08-04/text/original/epub/OEBPS/document_1/document_1.html#_Toc143507952"^^xsd:anyURI ;
    dcat:theme legcons:Item .

F2021L00334:307 a legcons:Item,
        owl:Class,
        dcat:Resource ;
    rdfs:label "Item - I307 8 37  Purpose of this Division"@en-AU ;
    dct:isPartOf F2021L00334:306 ;
    dct:isReferencedBy F2021L00334: ;
    rdfs:comment "8 37  Purpose of this Division - Abrievated Graph Key: I307"@en-AU ;
    skos:definition "8 37  Purpose of this Division"@en-AU ;
    skos:narrower F2021L00334:306 ;
    skos:prefLabel "Item I307"@en-AU ;
    dcat:accessURL <https://www.legislation.gov.au/F2021L00334/2023-08-04/2023-08-04/text/original/epub/OEBPS/document_1/document_1.html#_Toc143507954> ;
    dcat:landingPage "https://www.legislation.gov.au/F2021L00334/2023-08-04/2023-08-04/text/original/epub/OEBPS/document_1/document_1.html#_Toc143507954"^^xsd:anyURI ;
    dcat:theme legcons:Item .

F2021L00334:308 a legcons:Item,
        owl:Class,
        dcat:Resource ;
    rdfs:label "Item - I308 8 38  Persons who may manufacture supply or possess official marking devices"@en-AU ;
    dct:isPartOf F2021L00334:306 ;
    dct:isReferencedBy F2021L00334: ;
    rdfs:comment "8 38  Persons who may manufacture supply or possess official marking devices - Abrievated Graph Key: I308"@en-AU ;
    skos:definition "8 38  Persons who may manufacture supply or possess official marking devices"@en-AU ;
    skos:narrower F2021L00334:306 ;
    skos:prefLabel "Item I308"@en-AU ;
    dcat:accessURL <https://www.legislation.gov.au/F2021L00334/2023-08-04/2023-08-04/text/original/epub/OEBPS/document_1/document_1.html#_Toc143507955> ;
    dcat:landingPage "https://www.legislation.gov.au/F2021L00334/2023-08-04/2023-08-04/text/original/epub/OEBPS/document_1/document_1.html#_Toc143507955"^^xsd:anyURI ;
    dcat:theme legcons:Item .

F2021L00334:309 a legcons:Item,
        owl:Class,
        dcat:Resource ;
    rdfs:label "Item - I309 8 39  Security of official marking devices"@en-AU ;
    dct:isPartOf F2021L00334:306 ;
    dct:isReferencedBy F2021L00334: ;
    rdfs:comment "8 39  Security of official marking devices - Abrievated Graph Key: I309"@en-AU ;
    skos:definition "8 39  Security of official marking devices"@en-AU ;
    skos:narrower F2021L00334:306 ;
    skos:prefLabel "Item I309"@en-AU ;
    dcat:accessURL <https://www.legislation.gov.au/F2021L00334/2023-08-04/2023-08-04/text/original/epub/OEBPS/document_1/document_1.html#_Toc143507956> ;
    dcat:landingPage "https://www.legislation.gov.au/F2021L00334/2023-08-04/2023-08-04/text/original/epub/OEBPS/document_1/document_1.html#_Toc143507956"^^xsd:anyURI ;
    dcat:theme legcons:Item .

F2021L00334:31 a legcons:Item,
        owl:Class,
        dcat:Resource ;
    rdfs:label "Item - I31 2 12  Halal certificates"@en-AU ;
    dct:isPartOf F2021L00334:29 ;
    dct:isReferencedBy F2021L00334: ;
    rdfs:comment "2 12  Halal certificates - Abrievated Graph Key: I31"@en-AU ;
    skos:definition "2 12  Halal certificates"@en-AU ;
    skos:narrower F2021L00334:29 ;
    skos:prefLabel "Item I31"@en-AU ;
    dcat:accessURL <https://www.legislation.gov.au/F2021L00334/2023-08-04/2023-08-04/text/original/epub/OEBPS/document_1/document_1.html#_Toc143507678> ;
    dcat:landingPage "https://www.legislation.gov.au/F2021L00334/2023-08-04/2023-08-04/text/original/epub/OEBPS/document_1/document_1.html#_Toc143507678"^^xsd:anyURI ;
    dcat:theme legcons:Item .

F2021L00334:310 a legcons:Item,
        owl:Class,
        dcat:Resource ;
    rdfs:label "Item - I310 8 40  Damaged etc official marking devices"@en-AU ;
    dct:isPartOf F2021L00334:306 ;
    dct:isReferencedBy F2021L00334: ;
    rdfs:comment "8 40  Damaged etc official marking devices - Abrievated Graph Key: I310"@en-AU ;
    skos:definition "8 40  Damaged etc official marking devices"@en-AU ;
    skos:narrower F2021L00334:306 ;
    skos:prefLabel "Item I310"@en-AU ;
    dcat:accessURL <https://www.legislation.gov.au/F2021L00334/2023-08-04/2023-08-04/text/original/epub/OEBPS/document_1/document_1.html#_Toc143507957> ;
    dcat:landingPage "https://www.legislation.gov.au/F2021L00334/2023-08-04/2023-08-04/text/original/epub/OEBPS/document_1/document_1.html#_Toc143507957"^^xsd:anyURI ;
    dcat:theme legcons:Item .

F2021L00334:311 a legcons:Item,
        owl:Class,
        dcat:Resource ;
    rdfs:label "Item - I311 8 41  Records of official marking devices manufactured or supplied"@en-AU ;
    dct:isPartOf F2021L00334:306 ;
    dct:isReferencedBy F2021L00334: ;
    rdfs:comment "8 41  Records of official marking devices manufactured or supplied - Abrievated Graph Key: I311"@en-AU ;
    skos:definition "8 41  Records of official marking devices manufactured or supplied"@en-AU ;
    skos:narrower F2021L00334:306 ;
    skos:prefLabel "Item I311"@en-AU ;
    dcat:accessURL <https://www.legislation.gov.au/F2021L00334/2023-08-04/2023-08-04/text/original/epub/OEBPS/document_1/document_1.html#_Toc143507958> ;
    dcat:landingPage "https://www.legislation.gov.au/F2021L00334/2023-08-04/2023-08-04/text/original/epub/OEBPS/document_1/document_1.html#_Toc143507958"^^xsd:anyURI ;
    dcat:theme legcons:Item .

F2021L00334:312 a legcons:Item,
        owl:Class,
        dcat:Resource ;
    rdfs:label "Item - I312 8 42  Records of official marking devices received used damaged destroyed or returned"@en-AU ;
    dct:isPartOf F2021L00334:306 ;
    dct:isReferencedBy F2021L00334: ;
    rdfs:comment "8 42  Records of official marking devices received used damaged destroyed or returned - Abrievated Graph Key: I312"@en-AU ;
    skos:definition "8 42  Records of official marking devices received used damaged destroyed or returned"@en-AU ;
    skos:narrower F2021L00334:306 ;
    skos:prefLabel "Item I312"@en-AU ;
    dcat:accessURL <https://www.legislation.gov.au/F2021L00334/2023-08-04/2023-08-04/text/original/epub/OEBPS/document_1/document_1.html#_Toc143507959> ;
    dcat:landingPage "https://www.legislation.gov.au/F2021L00334/2023-08-04/2023-08-04/text/original/epub/OEBPS/document_1/document_1.html#_Toc143507959"^^xsd:anyURI ;
    dcat:theme legcons:Item .

F2021L00334:316 a legcons:Item,
        owl:Class,
        dcat:Resource ;
    rdfs:label "Item - I316 9 1  References to audit in this Part"@en-AU ;
    dct:isPartOf F2021L00334:315 ;
    dct:isReferencedBy F2021L00334: ;
    rdfs:comment "9 1  References to audit in this Part - Abrievated Graph Key: I316"@en-AU ;
    skos:definition "9 1  References to audit in this Part"@en-AU ;
    skos:narrower F2021L00334:315 ;
    skos:prefLabel "Item I316"@en-AU ;
    dcat:accessURL <https://www.legislation.gov.au/F2021L00334/2023-08-04/2023-08-04/text/original/epub/OEBPS/document_1/document_1.html#_Toc143507963> ;
    dcat:landingPage "https://www.legislation.gov.au/F2021L00334/2023-08-04/2023-08-04/text/original/epub/OEBPS/document_1/document_1.html#_Toc143507963"^^xsd:anyURI ;
    dcat:theme legcons:Item .

F2021L00334:318 a legcons:Item,
        owl:Class,
        dcat:Resource ;
    rdfs:label "Item - I318 9 2  Purpose of this Division"@en-AU ;
    dct:isPartOf F2021L00334:317 ;
    dct:isReferencedBy F2021L00334: ;
    rdfs:comment "9 2  Purpose of this Division - Abrievated Graph Key: I318"@en-AU ;
    skos:definition "9 2  Purpose of this Division"@en-AU ;
    skos:narrower F2021L00334:317 ;
    skos:prefLabel "Item I318"@en-AU ;
    dcat:accessURL <https://www.legislation.gov.au/F2021L00334/2023-08-04/2023-08-04/text/original/epub/OEBPS/document_1/document_1.html#_Toc143507965> ;
    dcat:landingPage "https://www.legislation.gov.au/F2021L00334/2023-08-04/2023-08-04/text/original/epub/OEBPS/document_1/document_1.html#_Toc143507965"^^xsd:anyURI ;
    dcat:theme legcons:Item .

F2021L00334:319 a legcons:Item,
        owl:Class,
        dcat:Resource ;
    rdfs:label "Item - I319 9 3  Manner in which audit must be conducted"@en-AU ;
    dct:isPartOf F2021L00334:317 ;
    dct:isReferencedBy F2021L00334: ;
    rdfs:comment "9 3  Manner in which audit must be conducted - Abrievated Graph Key: I319"@en-AU ;
    skos:definition "9 3  Manner in which audit must be conducted"@en-AU ;
    skos:narrower F2021L00334:317 ;
    skos:prefLabel "Item I319"@en-AU ;
    dcat:accessURL <https://www.legislation.gov.au/F2021L00334/2023-08-04/2023-08-04/text/original/epub/OEBPS/document_1/document_1.html#_Toc143507966> ;
    dcat:landingPage "https://www.legislation.gov.au/F2021L00334/2023-08-04/2023-08-04/text/original/epub/OEBPS/document_1/document_1.html#_Toc143507966"^^xsd:anyURI ;
    dcat:theme legcons:Item .

F2021L00334:32 a legcons:Item,
        owl:Class,
        dcat:Resource ;
    rdfs:label "Item - I32 2 13  Issuing bodies for Halal certificates"@en-AU ;
    dct:isPartOf F2021L00334:29 ;
    dct:isReferencedBy F2021L00334: ;
    rdfs:comment "2 13  Issuing bodies for Halal certificates - Abrievated Graph Key: I32"@en-AU ;
    skos:definition "2 13  Issuing bodies for Halal certificates"@en-AU ;
    skos:narrower F2021L00334:29 ;
    skos:prefLabel "Item I32"@en-AU ;
    dcat:accessURL <https://www.legislation.gov.au/F2021L00334/2023-08-04/2023-08-04/text/original/epub/OEBPS/document_1/document_1.html#_Toc143507679> ;
    dcat:landingPage "https://www.legislation.gov.au/F2021L00334/2023-08-04/2023-08-04/text/original/epub/OEBPS/document_1/document_1.html#_Toc143507679"^^xsd:anyURI ;
    dcat:theme legcons:Item .

F2021L00334:320 a legcons:Item,
        owl:Class,
        dcat:Resource ;
    rdfs:label "Item - I320 9 4  Notice of non compliance with requirements"@en-AU ;
    dct:isPartOf F2021L00334:317 ;
    dct:isReferencedBy F2021L00334: ;
    rdfs:comment "9 4  Notice of non compliance with requirements - Abrievated Graph Key: I320"@en-AU ;
    skos:definition "9 4  Notice of non compliance with requirements"@en-AU ;
    skos:narrower F2021L00334:317 ;
    skos:prefLabel "Item I320"@en-AU ;
    dcat:accessURL <https://www.legislation.gov.au/F2021L00334/2023-08-04/2023-08-04/text/original/epub/OEBPS/document_1/document_1.html#_Toc143507967> ;
    dcat:landingPage "https://www.legislation.gov.au/F2021L00334/2023-08-04/2023-08-04/text/original/epub/OEBPS/document_1/document_1.html#_Toc143507967"^^xsd:anyURI ;
    dcat:theme legcons:Item .

F2021L00334:321 a legcons:Item,
        owl:Class,
        dcat:Resource ;
    rdfs:label "Item - I321 9 5  Audit reports"@en-AU ;
    dct:isPartOf F2021L00334:317 ;
    dct:isReferencedBy F2021L00334: ;
    rdfs:comment "9 5  Audit reports - Abrievated Graph Key: I321"@en-AU ;
    skos:definition "9 5  Audit reports"@en-AU ;
    skos:narrower F2021L00334:317 ;
    skos:prefLabel "Item I321"@en-AU ;
    dcat:accessURL <https://www.legislation.gov.au/F2021L00334/2023-08-04/2023-08-04/text/original/epub/OEBPS/document_1/document_1.html#_Toc143507968> ;
    dcat:landingPage "https://www.legislation.gov.au/F2021L00334/2023-08-04/2023-08-04/text/original/epub/OEBPS/document_1/document_1.html#_Toc143507968"^^xsd:anyURI ;
    dcat:theme legcons:Item .

F2021L00334:323 a legcons:Item,
        owl:Class,
        dcat:Resource ;
    rdfs:label "Item - I323 9 6  Purpose of this Division"@en-AU ;
    dct:isPartOf F2021L00334:322 ;
    dct:isReferencedBy F2021L00334: ;
    rdfs:comment "9 6  Purpose of this Division - Abrievated Graph Key: I323"@en-AU ;
    skos:definition "9 6  Purpose of this Division"@en-AU ;
    skos:narrower F2021L00334:322 ;
    skos:prefLabel "Item I323"@en-AU ;
    dcat:accessURL <https://www.legislation.gov.au/F2021L00334/2023-08-04/2023-08-04/text/original/epub/OEBPS/document_1/document_1.html#_Toc143507970> ;
    dcat:landingPage "https://www.legislation.gov.au/F2021L00334/2023-08-04/2023-08-04/text/original/epub/OEBPS/document_1/document_1.html#_Toc143507970"^^xsd:anyURI ;
    dcat:theme legcons:Item .

F2021L00334:324 a legcons:Item,
        owl:Class,
        dcat:Resource ;
    rdfs:label "Item - I324 9 7  Application for approval"@en-AU ;
    dct:isPartOf F2021L00334:322 ;
    dct:isReferencedBy F2021L00334: ;
    rdfs:comment "9 7  Application for approval - Abrievated Graph Key: I324"@en-AU ;
    skos:definition "9 7  Application for approval"@en-AU ;
    skos:narrower F2021L00334:322 ;
    skos:prefLabel "Item I324"@en-AU ;
    dcat:accessURL <https://www.legislation.gov.au/F2021L00334/2023-08-04/2023-08-04/text/original/epub/OEBPS/document_1/document_1.html#_Toc143507971> ;
    dcat:landingPage "https://www.legislation.gov.au/F2021L00334/2023-08-04/2023-08-04/text/original/epub/OEBPS/document_1/document_1.html#_Toc143507971"^^xsd:anyURI ;
    dcat:theme legcons:Item .

F2021L00334:325 a legcons:Item,
        owl:Class,
        dcat:Resource ;
    rdfs:label "Item - I325 9 8  Secretary must decide whether to approve applicant to conduct audits"@en-AU ;
    dct:isPartOf F2021L00334:322 ;
    dct:isReferencedBy F2021L00334: ;
    rdfs:comment "9 8  Secretary must decide whether to approve applicant to conduct audits - Abrievated Graph Key: I325"@en-AU ;
    skos:definition "9 8  Secretary must decide whether to approve applicant to conduct audits"@en-AU ;
    skos:narrower F2021L00334:322 ;
    skos:prefLabel "Item I325"@en-AU ;
    dcat:accessURL <https://www.legislation.gov.au/F2021L00334/2023-08-04/2023-08-04/text/original/epub/OEBPS/document_1/document_1.html#_Toc143507972> ;
    dcat:landingPage "https://www.legislation.gov.au/F2021L00334/2023-08-04/2023-08-04/text/original/epub/OEBPS/document_1/document_1.html#_Toc143507972"^^xsd:anyURI ;
    dcat:theme legcons:Item .

F2021L00334:326 a legcons:Item,
        owl:Class,
        dcat:Resource ;
    rdfs:label "Item - I326 9 9  Dealing with applications"@en-AU ;
    dct:isPartOf F2021L00334:322 ;
    dct:isReferencedBy F2021L00334: ;
    rdfs:comment "9 9  Dealing with applications - Abrievated Graph Key: I326"@en-AU ;
    skos:definition "9 9  Dealing with applications"@en-AU ;
    skos:narrower F2021L00334:322 ;
    skos:prefLabel "Item I326"@en-AU ;
    dcat:accessURL <https://www.legislation.gov.au/F2021L00334/2023-08-04/2023-08-04/text/original/epub/OEBPS/document_1/document_1.html#_Toc143507973> ;
    dcat:landingPage "https://www.legislation.gov.au/F2021L00334/2023-08-04/2023-08-04/text/original/epub/OEBPS/document_1/document_1.html#_Toc143507973"^^xsd:anyURI ;
    dcat:theme legcons:Item .

F2021L00334:327 a legcons:Item,
        owl:Class,
        dcat:Resource ;
    rdfs:label "Item - I327 9 10  Conditions of approval"@en-AU ;
    dct:isPartOf F2021L00334:322 ;
    dct:isReferencedBy F2021L00334: ;
    rdfs:comment "9 10  Conditions of approval - Abrievated Graph Key: I327"@en-AU ;
    skos:definition "9 10  Conditions of approval"@en-AU ;
    skos:narrower F2021L00334:322 ;
    skos:prefLabel "Item I327"@en-AU ;
    dcat:accessURL <https://www.legislation.gov.au/F2021L00334/2023-08-04/2023-08-04/text/original/epub/OEBPS/document_1/document_1.html#_Toc143507974> ;
    dcat:landingPage "https://www.legislation.gov.au/F2021L00334/2023-08-04/2023-08-04/text/original/epub/OEBPS/document_1/document_1.html#_Toc143507974"^^xsd:anyURI ;
    dcat:theme legcons:Item .

F2021L00334:328 a legcons:Item,
        owl:Class,
        dcat:Resource ;
    rdfs:label "Item - I328 9 11  Notice of decision"@en-AU ;
    dct:isPartOf F2021L00334:322 ;
    dct:isReferencedBy F2021L00334: ;
    rdfs:comment "9 11  Notice of decision - Abrievated Graph Key: I328"@en-AU ;
    skos:definition "9 11  Notice of decision"@en-AU ;
    skos:narrower F2021L00334:322 ;
    skos:prefLabel "Item I328"@en-AU ;
    dcat:accessURL <https://www.legislation.gov.au/F2021L00334/2023-08-04/2023-08-04/text/original/epub/OEBPS/document_1/document_1.html#_Toc143507975> ;
    dcat:landingPage "https://www.legislation.gov.au/F2021L00334/2023-08-04/2023-08-04/text/original/epub/OEBPS/document_1/document_1.html#_Toc143507975"^^xsd:anyURI ;
    dcat:theme legcons:Item .

F2021L00334:329 a legcons:Item,
        owl:Class,
        dcat:Resource ;
    rdfs:label "Item - I329 9 12  Period of effect of approval"@en-AU ;
    dct:isPartOf F2021L00334:322 ;
    dct:isReferencedBy F2021L00334: ;
    rdfs:comment "9 12  Period of effect of approval - Abrievated Graph Key: I329"@en-AU ;
    skos:definition "9 12  Period of effect of approval"@en-AU ;
    skos:narrower F2021L00334:322 ;
    skos:prefLabel "Item I329"@en-AU ;
    dcat:accessURL <https://www.legislation.gov.au/F2021L00334/2023-08-04/2023-08-04/text/original/epub/OEBPS/document_1/document_1.html#_Toc143507976> ;
    dcat:landingPage "https://www.legislation.gov.au/F2021L00334/2023-08-04/2023-08-04/text/original/epub/OEBPS/document_1/document_1.html#_Toc143507976"^^xsd:anyURI ;
    dcat:theme legcons:Item .

F2021L00334:33 a legcons:Item,
        owl:Class,
        dcat:Resource ;
    rdfs:label "Item - I33 2 14  Declaration to accompany application for government certificate"@en-AU ;
    dct:isPartOf F2021L00334:29 ;
    dct:isReferencedBy F2021L00334: ;
    rdfs:comment "2 14  Declaration to accompany application for government certificate - Abrievated Graph Key: I33"@en-AU ;
    skos:definition "2 14  Declaration to accompany application for government certificate"@en-AU ;
    skos:narrower F2021L00334:29 ;
    skos:prefLabel "Item I33"@en-AU ;
    dcat:accessURL <https://www.legislation.gov.au/F2021L00334/2023-08-04/2023-08-04/text/original/epub/OEBPS/document_1/document_1.html#_Toc143507680> ;
    dcat:landingPage "https://www.legislation.gov.au/F2021L00334/2023-08-04/2023-08-04/text/original/epub/OEBPS/document_1/document_1.html#_Toc143507680"^^xsd:anyURI ;
    dcat:theme legcons:Item .

F2021L00334:330 a legcons:Item,
        owl:Class,
        dcat:Resource ;
    rdfs:label "Item - I330 9 13  Imposing or varying conditions of approval"@en-AU ;
    dct:isPartOf F2021L00334:322 ;
    dct:isReferencedBy F2021L00334: ;
    rdfs:comment "9 13  Imposing or varying conditions of approval - Abrievated Graph Key: I330"@en-AU ;
    skos:definition "9 13  Imposing or varying conditions of approval"@en-AU ;
    skos:narrower F2021L00334:322 ;
    skos:prefLabel "Item I330"@en-AU ;
    dcat:accessURL <https://www.legislation.gov.au/F2021L00334/2023-08-04/2023-08-04/text/original/epub/OEBPS/document_1/document_1.html#_Toc143507977> ;
    dcat:landingPage "https://www.legislation.gov.au/F2021L00334/2023-08-04/2023-08-04/text/original/epub/OEBPS/document_1/document_1.html#_Toc143507977"^^xsd:anyURI ;
    dcat:theme legcons:Item .

F2021L00334:331 a legcons:Item,
        owl:Class,
        dcat:Resource ;
    rdfs:label "Item - I331 9 14  Revocation of approval"@en-AU ;
    dct:isPartOf F2021L00334:322 ;
    dct:isReferencedBy F2021L00334: ;
    rdfs:comment "9 14  Revocation of approval - Abrievated Graph Key: I331"@en-AU ;
    skos:definition "9 14  Revocation of approval"@en-AU ;
    skos:narrower F2021L00334:322 ;
    skos:prefLabel "Item I331"@en-AU ;
    dcat:accessURL <https://www.legislation.gov.au/F2021L00334/2023-08-04/2023-08-04/text/original/epub/OEBPS/document_1/document_1.html#_Toc143507978> ;
    dcat:landingPage "https://www.legislation.gov.au/F2021L00334/2023-08-04/2023-08-04/text/original/epub/OEBPS/document_1/document_1.html#_Toc143507978"^^xsd:anyURI ;
    dcat:theme legcons:Item .

F2021L00334:332 a legcons:Item,
        owl:Class,
        dcat:Resource ;
    rdfs:label "Item - I332 9 15  Register of approved auditors"@en-AU ;
    dct:isPartOf F2021L00334:322 ;
    dct:isReferencedBy F2021L00334: ;
    rdfs:comment "9 15  Register of approved auditors - Abrievated Graph Key: I332"@en-AU ;
    skos:definition "9 15  Register of approved auditors"@en-AU ;
    skos:narrower F2021L00334:322 ;
    skos:prefLabel "Item I332"@en-AU ;
    dcat:accessURL <https://www.legislation.gov.au/F2021L00334/2023-08-04/2023-08-04/text/original/epub/OEBPS/document_1/document_1.html#_Toc143507979> ;
    dcat:landingPage "https://www.legislation.gov.au/F2021L00334/2023-08-04/2023-08-04/text/original/epub/OEBPS/document_1/document_1.html#_Toc143507979"^^xsd:anyURI ;
    dcat:theme legcons:Item .

F2021L00334:333 a legcons:Item,
        owl:Class,
        dcat:Resource ;
    rdfs:label "Item - I333 9 16  Fit and proper person test"@en-AU ;
    dct:isPartOf F2021L00334:322 ;
    dct:isReferencedBy F2021L00334: ;
    rdfs:comment "9 16  Fit and proper person test - Abrievated Graph Key: I333"@en-AU ;
    skos:definition "9 16  Fit and proper person test"@en-AU ;
    skos:narrower F2021L00334:322 ;
    skos:prefLabel "Item I333"@en-AU ;
    dcat:accessURL <https://www.legislation.gov.au/F2021L00334/2023-08-04/2023-08-04/text/original/epub/OEBPS/document_1/document_1.html#_Toc143507980> ;
    dcat:landingPage "https://www.legislation.gov.au/F2021L00334/2023-08-04/2023-08-04/text/original/epub/OEBPS/document_1/document_1.html#_Toc143507980"^^xsd:anyURI ;
    dcat:theme legcons:Item .

F2021L00334:335 a legcons:Item,
        owl:Class,
        dcat:Resource ;
    rdfs:label "Item - I335 9 17  Circumstances in which assessment may be required or permitted"@en-AU ;
    dct:isPartOf F2021L00334:334 ;
    dct:isReferencedBy F2021L00334: ;
    rdfs:comment "9 17  Circumstances in which assessment may be required or permitted - Abrievated Graph Key: I335"@en-AU ;
    skos:definition "9 17  Circumstances in which assessment may be required or permitted"@en-AU ;
    skos:narrower F2021L00334:334 ;
    skos:prefLabel "Item I335"@en-AU ;
    dcat:accessURL <https://www.legislation.gov.au/F2021L00334/2023-08-04/2023-08-04/text/original/epub/OEBPS/document_1/document_1.html#_Toc143507982> ;
    dcat:landingPage "https://www.legislation.gov.au/F2021L00334/2023-08-04/2023-08-04/text/original/epub/OEBPS/document_1/document_1.html#_Toc143507982"^^xsd:anyURI ;
    dcat:theme legcons:Item .

F2021L00334:337 a legcons:Item,
        owl:Class,
        dcat:Resource ;
    rdfs:label "Item - I337 9 18  Decisions that may be made by operation of computer program"@en-AU ;
    dct:isPartOf F2021L00334:336 ;
    dct:isReferencedBy F2021L00334: ;
    rdfs:comment "9 18  Decisions that may be made by operation of computer program - Abrievated Graph Key: I337"@en-AU ;
    skos:definition "9 18  Decisions that may be made by operation of computer program"@en-AU ;
    skos:narrower F2021L00334:336 ;
    skos:prefLabel "Item I337"@en-AU ;
    dcat:accessURL <https://www.legislation.gov.au/F2021L00334/2023-08-04/2023-08-04/text/original/epub/OEBPS/document_1/document_1.html#_Toc143507984> ;
    dcat:landingPage "https://www.legislation.gov.au/F2021L00334/2023-08-04/2023-08-04/text/original/epub/OEBPS/document_1/document_1.html#_Toc143507984"^^xsd:anyURI ;
    dcat:theme legcons:Item .

F2021L00334:34 a legcons:Item,
        owl:Class,
        dcat:Resource ;
    rdfs:label "Item - I34 2 15  Circumstances for refusing to issue government certificate"@en-AU ;
    dct:isPartOf F2021L00334:29 ;
    dct:isReferencedBy F2021L00334: ;
    rdfs:comment "2 15  Circumstances for refusing to issue government certificate - Abrievated Graph Key: I34"@en-AU ;
    skos:definition "2 15  Circumstances for refusing to issue government certificate"@en-AU ;
    skos:narrower F2021L00334:29 ;
    skos:prefLabel "Item I34"@en-AU ;
    dcat:accessURL <https://www.legislation.gov.au/F2021L00334/2023-08-04/2023-08-04/text/original/epub/OEBPS/document_1/document_1.html#_Toc143507681> ;
    dcat:landingPage "https://www.legislation.gov.au/F2021L00334/2023-08-04/2023-08-04/text/original/epub/OEBPS/document_1/document_1.html#_Toc143507681"^^xsd:anyURI ;
    dcat:theme legcons:Item .

F2021L00334:340 a legcons:Item,
        owl:Class,
        dcat:Resource ;
    rdfs:label "Item - I340 9 19  Requirement to be third party authorised officerfit and proper person etc"@en-AU ;
    dct:isPartOf F2021L00334:339 ;
    dct:isReferencedBy F2021L00334: ;
    rdfs:comment "9 19  Requirement to be third party authorised officerfit and proper person etc - Abrievated Graph Key: I340"@en-AU ;
    skos:definition "9 19  Requirement to be third party authorised officerfit and proper person etc"@en-AU ;
    skos:narrower F2021L00334:339 ;
    skos:prefLabel "Item I340"@en-AU ;
    dcat:accessURL <https://www.legislation.gov.au/F2021L00334/2023-08-04/2023-08-04/text/original/epub/OEBPS/document_1/document_1.html#_Toc143507987> ;
    dcat:landingPage "https://www.legislation.gov.au/F2021L00334/2023-08-04/2023-08-04/text/original/epub/OEBPS/document_1/document_1.html#_Toc143507987"^^xsd:anyURI ;
    dcat:theme legcons:Item .

F2021L00334:342 a legcons:Item,
        owl:Class,
        dcat:Resource ;
    rdfs:label "Item - I342 9 20  Purpose of this Division"@en-AU ;
    dct:isPartOf F2021L00334:341 ;
    dct:isReferencedBy F2021L00334: ;
    rdfs:comment "9 20  Purpose of this Division - Abrievated Graph Key: I342"@en-AU ;
    skos:definition "9 20  Purpose of this Division"@en-AU ;
    skos:narrower F2021L00334:341 ;
    skos:prefLabel "Item I342"@en-AU ;
    dcat:accessURL <https://www.legislation.gov.au/F2021L00334/2023-08-04/2023-08-04/text/original/epub/OEBPS/document_1/document_1.html#_Toc143507989> ;
    dcat:landingPage "https://www.legislation.gov.au/F2021L00334/2023-08-04/2023-08-04/text/original/epub/OEBPS/document_1/document_1.html#_Toc143507989"^^xsd:anyURI ;
    dcat:theme legcons:Item .

F2021L00334:343 a legcons:Item,
        owl:Class,
        dcat:Resource ;
    rdfs:label "Item - I343 9 21  Functions specified in Australian Meat Standard"@en-AU ;
    dct:isPartOf F2021L00334:341 ;
    dct:isReferencedBy F2021L00334: ;
    rdfs:comment "9 21  Functions specified in Australian Meat Standard - Abrievated Graph Key: I343"@en-AU ;
    skos:definition "9 21  Functions specified in Australian Meat Standard"@en-AU ;
    skos:narrower F2021L00334:341 ;
    skos:prefLabel "Item I343"@en-AU ;
    dcat:accessURL <https://www.legislation.gov.au/F2021L00334/2023-08-04/2023-08-04/text/original/epub/OEBPS/document_1/document_1.html#_Toc143507990> ;
    dcat:landingPage "https://www.legislation.gov.au/F2021L00334/2023-08-04/2023-08-04/text/original/epub/OEBPS/document_1/document_1.html#_Toc143507990"^^xsd:anyURI ;
    dcat:theme legcons:Item .

F2021L00334:344 a legcons:Item,
        owl:Class,
        dcat:Resource ;
    rdfs:label "Item - I344 9 22  Applying admission decisions"@en-AU ;
    dct:isPartOf F2021L00334:341 ;
    dct:isReferencedBy F2021L00334: ;
    rdfs:comment "9 22  Applying admission decisions - Abrievated Graph Key: I344"@en-AU ;
    skos:definition "9 22  Applying admission decisions"@en-AU ;
    skos:narrower F2021L00334:341 ;
    skos:prefLabel "Item I344"@en-AU ;
    dcat:accessURL <https://www.legislation.gov.au/F2021L00334/2023-08-04/2023-08-04/text/original/epub/OEBPS/document_1/document_1.html#_Toc143507991> ;
    dcat:landingPage "https://www.legislation.gov.au/F2021L00334/2023-08-04/2023-08-04/text/original/epub/OEBPS/document_1/document_1.html#_Toc143507991"^^xsd:anyURI ;
    dcat:theme legcons:Item .

F2021L00334:345 a legcons:Item,
        owl:Class,
        dcat:Resource ;
    rdfs:label "Item - I345 9 23  Inspections of animals for slaughter and applying ante mortem dispositions"@en-AU ;
    dct:isPartOf F2021L00334:341 ;
    dct:isReferencedBy F2021L00334: ;
    rdfs:comment "9 23  Inspections of animals for slaughter and applying ante mortem dispositions - Abrievated Graph Key: I345"@en-AU ;
    skos:definition "9 23  Inspections of animals for slaughter and applying ante mortem dispositions"@en-AU ;
    skos:narrower F2021L00334:341 ;
    skos:prefLabel "Item I345"@en-AU ;
    dcat:accessURL <https://www.legislation.gov.au/F2021L00334/2023-08-04/2023-08-04/text/original/epub/OEBPS/document_1/document_1.html#_Toc143507992> ;
    dcat:landingPage "https://www.legislation.gov.au/F2021L00334/2023-08-04/2023-08-04/text/original/epub/OEBPS/document_1/document_1.html#_Toc143507992"^^xsd:anyURI ;
    dcat:theme legcons:Item .

F2021L00334:346 a legcons:Item,
        owl:Class,
        dcat:Resource ;
    rdfs:label "Item - I346 9 24  Inspections of carcases and carcase parts and applying post mortem dispositions"@en-AU ;
    dct:isPartOf F2021L00334:341 ;
    dct:isReferencedBy F2021L00334: ;
    rdfs:comment "9 24  Inspections of carcases and carcase parts and applying post mortem dispositions - Abrievated Graph Key: I346"@en-AU ;
    skos:definition "9 24  Inspections of carcases and carcase parts and applying post mortem dispositions"@en-AU ;
    skos:narrower F2021L00334:341 ;
    skos:prefLabel "Item I346"@en-AU ;
    dcat:accessURL <https://www.legislation.gov.au/F2021L00334/2023-08-04/2023-08-04/text/original/epub/OEBPS/document_1/document_1.html#_Toc143507993> ;
    dcat:landingPage "https://www.legislation.gov.au/F2021L00334/2023-08-04/2023-08-04/text/original/epub/OEBPS/document_1/document_1.html#_Toc143507993"^^xsd:anyURI ;
    dcat:theme legcons:Item .

F2021L00334:347 a legcons:Item,
        owl:Class,
        dcat:Resource ;
    rdfs:label "Item - I347 9 25  Inspections of meat and meat products and applying dispositions"@en-AU ;
    dct:isPartOf F2021L00334:341 ;
    dct:isReferencedBy F2021L00334: ;
    rdfs:comment "9 25  Inspections of meat and meat products and applying dispositions - Abrievated Graph Key: I347"@en-AU ;
    skos:definition "9 25  Inspections of meat and meat products and applying dispositions"@en-AU ;
    skos:narrower F2021L00334:341 ;
    skos:prefLabel "Item I347"@en-AU ;
    dcat:accessURL <https://www.legislation.gov.au/F2021L00334/2023-08-04/2023-08-04/text/original/epub/OEBPS/document_1/document_1.html#_Toc143507994> ;
    dcat:landingPage "https://www.legislation.gov.au/F2021L00334/2023-08-04/2023-08-04/text/original/epub/OEBPS/document_1/document_1.html#_Toc143507994"^^xsd:anyURI ;
    dcat:theme legcons:Item .

F2021L00334:348 a legcons:Item,
        owl:Class,
        dcat:Resource ;
    rdfs:label "Item - I348 9 26  Applying decisions or dispositions subject to conditions and variation"@en-AU ;
    dct:isPartOf F2021L00334:341 ;
    dct:isReferencedBy F2021L00334: ;
    rdfs:comment "9 26  Applying decisions or dispositions subject to conditions and variation - Abrievated Graph Key: I348"@en-AU ;
    skos:definition "9 26  Applying decisions or dispositions subject to conditions and variation"@en-AU ;
    skos:narrower F2021L00334:341 ;
    skos:prefLabel "Item I348"@en-AU ;
    dcat:accessURL <https://www.legislation.gov.au/F2021L00334/2023-08-04/2023-08-04/text/original/epub/OEBPS/document_1/document_1.html#_Toc143507995> ;
    dcat:landingPage "https://www.legislation.gov.au/F2021L00334/2023-08-04/2023-08-04/text/original/epub/OEBPS/document_1/document_1.html#_Toc143507995"^^xsd:anyURI ;
    dcat:theme legcons:Item .

F2021L00334:349 a legcons:Item,
        owl:Class,
        dcat:Resource ;
    rdfs:label "Item - I349 9 27  Stopping chain of operations temporarily or controlling rate of operations"@en-AU ;
    dct:isPartOf F2021L00334:341 ;
    dct:isReferencedBy F2021L00334: ;
    rdfs:comment "9 27  Stopping chain of operations temporarily or controlling rate of operations - Abrievated Graph Key: I349"@en-AU ;
    skos:definition "9 27  Stopping chain of operations temporarily or controlling rate of operations"@en-AU ;
    skos:narrower F2021L00334:341 ;
    skos:prefLabel "Item I349"@en-AU ;
    dcat:accessURL <https://www.legislation.gov.au/F2021L00334/2023-08-04/2023-08-04/text/original/epub/OEBPS/document_1/document_1.html#_Toc143507996> ;
    dcat:landingPage "https://www.legislation.gov.au/F2021L00334/2023-08-04/2023-08-04/text/original/epub/OEBPS/document_1/document_1.html#_Toc143507996"^^xsd:anyURI ;
    dcat:theme legcons:Item .

F2021L00334:35 a legcons:Item,
        owl:Class,
        dcat:Resource ;
    rdfs:label "Item - I35 2 16  Changes that require holder of certificate to give additional or corrected information to the issuing body"@en-AU ;
    dct:isPartOf F2021L00334:29 ;
    dct:isReferencedBy F2021L00334: ;
    rdfs:comment "2 16  Changes that require holder of certificate to give additional or corrected information to the issuing body - Abrievated Graph Key: I35"@en-AU ;
    skos:definition "2 16  Changes that require holder of certificate to give additional or corrected information to the issuing body"@en-AU ;
    skos:narrower F2021L00334:29 ;
    skos:prefLabel "Item I35"@en-AU ;
    dcat:accessURL <https://www.legislation.gov.au/F2021L00334/2023-08-04/2023-08-04/text/original/epub/OEBPS/document_1/document_1.html#_Toc143507682> ;
    dcat:landingPage "https://www.legislation.gov.au/F2021L00334/2023-08-04/2023-08-04/text/original/epub/OEBPS/document_1/document_1.html#_Toc143507682"^^xsd:anyURI ;
    dcat:theme legcons:Item .

F2021L00334:350 a legcons:Item,
        owl:Class,
        dcat:Resource ;
    rdfs:label "Item - I350 9 28  Functions to be performed by veterinary officer or authorised officer acting under supervision of veterinary officer"@en-AU ;
    dct:isPartOf F2021L00334:341 ;
    dct:isReferencedBy F2021L00334: ;
    rdfs:comment "9 28  Functions to be performed by veterinary officer or authorised officer acting under supervision of veterinary officer - Abrievated Graph Key: I350"@en-AU ;
    skos:definition "9 28  Functions to be performed by veterinary officer or authorised officer acting under supervision of veterinary officer"@en-AU ;
    skos:narrower F2021L00334:341 ;
    skos:prefLabel "Item I350"@en-AU ;
    dcat:accessURL <https://www.legislation.gov.au/F2021L00334/2023-08-04/2023-08-04/text/original/epub/OEBPS/document_1/document_1.html#_Toc143507997> ;
    dcat:landingPage "https://www.legislation.gov.au/F2021L00334/2023-08-04/2023-08-04/text/original/epub/OEBPS/document_1/document_1.html#_Toc143507997"^^xsd:anyURI ;
    dcat:theme legcons:Item .

F2021L00334:351 a legcons:Item,
        owl:Class,
        dcat:Resource ;
    rdfs:label "Item - I351 9 29  Inspecting establishments and securing areas facilities equipment or other things"@en-AU ;
    dct:isPartOf F2021L00334:341 ;
    dct:isReferencedBy F2021L00334: ;
    rdfs:comment "9 29  Inspecting establishments and securing areas facilities equipment or other things - Abrievated Graph Key: I351"@en-AU ;
    skos:definition "9 29  Inspecting establishments and securing areas facilities equipment or other things"@en-AU ;
    skos:narrower F2021L00334:341 ;
    skos:prefLabel "Item I351"@en-AU ;
    dcat:accessURL <https://www.legislation.gov.au/F2021L00334/2023-08-04/2023-08-04/text/original/epub/OEBPS/document_1/document_1.html#_Toc143507998> ;
    dcat:landingPage "https://www.legislation.gov.au/F2021L00334/2023-08-04/2023-08-04/text/original/epub/OEBPS/document_1/document_1.html#_Toc143507998"^^xsd:anyURI ;
    dcat:theme legcons:Item .

F2021L00334:352 a legcons:Item,
        owl:Class,
        dcat:Resource ;
    rdfs:label "Item - I352 9 30  Securing and identifying establishment or conveyance etc"@en-AU ;
    dct:isPartOf F2021L00334:341 ;
    dct:isReferencedBy F2021L00334: ;
    rdfs:comment "9 30  Securing and identifying establishment or conveyance etc - Abrievated Graph Key: I352"@en-AU ;
    skos:definition "9 30  Securing and identifying establishment or conveyance etc"@en-AU ;
    skos:narrower F2021L00334:341 ;
    skos:prefLabel "Item I352"@en-AU ;
    dcat:accessURL <https://www.legislation.gov.au/F2021L00334/2023-08-04/2023-08-04/text/original/epub/OEBPS/document_1/document_1.html#_Toc143507999> ;
    dcat:landingPage "https://www.legislation.gov.au/F2021L00334/2023-08-04/2023-08-04/text/original/epub/OEBPS/document_1/document_1.html#_Toc143507999"^^xsd:anyURI ;
    dcat:theme legcons:Item .

F2021L00334:353 a legcons:Item,
        owl:Class,
        dcat:Resource ;
    rdfs:label "Item - I353 9 31  Interference with identified establishment or conveyance etc"@en-AU ;
    dct:isPartOf F2021L00334:341 ;
    dct:isReferencedBy F2021L00334: ;
    rdfs:comment "9 31  Interference with identified establishment or conveyance etc - Abrievated Graph Key: I353"@en-AU ;
    skos:definition "9 31  Interference with identified establishment or conveyance etc"@en-AU ;
    skos:narrower F2021L00334:341 ;
    skos:prefLabel "Item I353"@en-AU ;
    dcat:accessURL <https://www.legislation.gov.au/F2021L00334/2023-08-04/2023-08-04/text/original/epub/OEBPS/document_1/document_1.html#_Toc143508000> ;
    dcat:landingPage "https://www.legislation.gov.au/F2021L00334/2023-08-04/2023-08-04/text/original/epub/OEBPS/document_1/document_1.html#_Toc143508000"^^xsd:anyURI ;
    dcat:theme legcons:Item .

F2021L00334:354 a legcons:Item,
        owl:Class,
        dcat:Resource ;
    rdfs:label "Item - I354 9 32  Powers where integrity of prescribed meat or meat products may not be able to be ensured"@en-AU ;
    dct:isPartOf F2021L00334:341 ;
    dct:isReferencedBy F2021L00334: ;
    rdfs:comment "9 32  Powers where integrity of prescribed meat or meat products may not be able to be ensured - Abrievated Graph Key: I354"@en-AU ;
    skos:definition "9 32  Powers where integrity of prescribed meat or meat products may not be able to be ensured"@en-AU ;
    skos:narrower F2021L00334:341 ;
    skos:prefLabel "Item I354"@en-AU ;
    dcat:accessURL <https://www.legislation.gov.au/F2021L00334/2023-08-04/2023-08-04/text/original/epub/OEBPS/document_1/document_1.html#_Toc143508001> ;
    dcat:landingPage "https://www.legislation.gov.au/F2021L00334/2023-08-04/2023-08-04/text/original/epub/OEBPS/document_1/document_1.html#_Toc143508001"^^xsd:anyURI ;
    dcat:theme legcons:Item .

F2021L00334:355 a legcons:Item,
        owl:Class,
        dcat:Resource ;
    rdfs:label "Item - I355 9 33  Giving certificate of condemnation"@en-AU ;
    dct:isPartOf F2021L00334:341 ;
    dct:isReferencedBy F2021L00334: ;
    rdfs:comment "9 33  Giving certificate of condemnation - Abrievated Graph Key: I355"@en-AU ;
    skos:definition "9 33  Giving certificate of condemnation"@en-AU ;
    skos:narrower F2021L00334:341 ;
    skos:prefLabel "Item I355"@en-AU ;
    dcat:accessURL <https://www.legislation.gov.au/F2021L00334/2023-08-04/2023-08-04/text/original/epub/OEBPS/document_1/document_1.html#_Toc143508002> ;
    dcat:landingPage "https://www.legislation.gov.au/F2021L00334/2023-08-04/2023-08-04/text/original/epub/OEBPS/document_1/document_1.html#_Toc143508002"^^xsd:anyURI ;
    dcat:theme legcons:Item .

F2021L00334:357 a legcons:Item,
        owl:Class,
        dcat:Resource ;
    rdfs:label "Item - I357 9 34  Other grounds for giving direction"@en-AU ;
    dct:isPartOf F2021L00334:356 ;
    dct:isReferencedBy F2021L00334: ;
    rdfs:comment "9 34  Other grounds for giving direction - Abrievated Graph Key: I357"@en-AU ;
    skos:definition "9 34  Other grounds for giving direction"@en-AU ;
    skos:narrower F2021L00334:356 ;
    skos:prefLabel "Item I357"@en-AU ;
    dcat:accessURL <https://www.legislation.gov.au/F2021L00334/2023-08-04/2023-08-04/text/original/epub/OEBPS/document_1/document_1.html#_Toc143508004> ;
    dcat:landingPage "https://www.legislation.gov.au/F2021L00334/2023-08-04/2023-08-04/text/original/epub/OEBPS/document_1/document_1.html#_Toc143508004"^^xsd:anyURI ;
    dcat:theme legcons:Item .

F2021L00334:359 a legcons:Item,
        owl:Class,
        dcat:Resource ;
    rdfs:label "Item - I359 9 35  Circumstances in which identity card need not be carried"@en-AU ;
    dct:isPartOf F2021L00334:358 ;
    dct:isReferencedBy F2021L00334: ;
    rdfs:comment "9 35  Circumstances in which identity card need not be carried - Abrievated Graph Key: I359"@en-AU ;
    skos:definition "9 35  Circumstances in which identity card need not be carried"@en-AU ;
    skos:narrower F2021L00334:358 ;
    skos:prefLabel "Item I359"@en-AU ;
    dcat:accessURL <https://www.legislation.gov.au/F2021L00334/2023-08-04/2023-08-04/text/original/epub/OEBPS/document_1/document_1.html#_Toc143508006> ;
    dcat:landingPage "https://www.legislation.gov.au/F2021L00334/2023-08-04/2023-08-04/text/original/epub/OEBPS/document_1/document_1.html#_Toc143508006"^^xsd:anyURI ;
    dcat:theme legcons:Item .

F2021L00334:36 a legcons:Item,
        owl:Class,
        dcat:Resource ;
    rdfs:label "Item - I36 2 17  Return of government certificate"@en-AU ;
    dct:isPartOf F2021L00334:29 ;
    dct:isReferencedBy F2021L00334: ;
    rdfs:comment "2 17  Return of government certificate - Abrievated Graph Key: I36"@en-AU ;
    skos:definition "2 17  Return of government certificate"@en-AU ;
    skos:narrower F2021L00334:29 ;
    skos:prefLabel "Item I36"@en-AU ;
    dcat:accessURL <https://www.legislation.gov.au/F2021L00334/2023-08-04/2023-08-04/text/original/epub/OEBPS/document_1/document_1.html#_Toc143507683> ;
    dcat:landingPage "https://www.legislation.gov.au/F2021L00334/2023-08-04/2023-08-04/text/original/epub/OEBPS/document_1/document_1.html#_Toc143507683"^^xsd:anyURI ;
    dcat:theme legcons:Item .

F2021L00334:361 a legcons:Item,
        owl:Class,
        dcat:Resource ;
    rdfs:label "Item - I361 10 1  Samples taken in exercising monitoring or investigation powers"@en-AU ;
    dct:isPartOf F2021L00334:360 ;
    dct:isReferencedBy F2021L00334: ;
    rdfs:comment "10 1  Samples taken in exercising monitoring or investigation powers - Abrievated Graph Key: I361"@en-AU ;
    skos:definition "10 1  Samples taken in exercising monitoring or investigation powers"@en-AU ;
    skos:narrower F2021L00334:360 ;
    skos:prefLabel "Item I361"@en-AU ;
    dcat:accessURL <https://www.legislation.gov.au/F2021L00334/2023-08-04/2023-08-04/text/original/epub/OEBPS/document_1/document_1.html#_Toc143508008> ;
    dcat:landingPage "https://www.legislation.gov.au/F2021L00334/2023-08-04/2023-08-04/text/original/epub/OEBPS/document_1/document_1.html#_Toc143508008"^^xsd:anyURI ;
    dcat:theme legcons:Item .

F2021L00334:362 a legcons:Item,
        owl:Class,
        dcat:Resource ;
    rdfs:label "Item - I362 10 2  Dealing with things seized in exercising investigation powers"@en-AU ;
    dct:isPartOf F2021L00334:360 ;
    dct:isReferencedBy F2021L00334: ;
    rdfs:comment "10 2  Dealing with things seized in exercising investigation powers - Abrievated Graph Key: I362"@en-AU ;
    skos:definition "10 2  Dealing with things seized in exercising investigation powers"@en-AU ;
    skos:narrower F2021L00334:360 ;
    skos:prefLabel "Item I362"@en-AU ;
    dcat:accessURL <https://www.legislation.gov.au/F2021L00334/2023-08-04/2023-08-04/text/original/epub/OEBPS/document_1/document_1.html#_Toc143508009> ;
    dcat:landingPage "https://www.legislation.gov.au/F2021L00334/2023-08-04/2023-08-04/text/original/epub/OEBPS/document_1/document_1.html#_Toc143508009"^^xsd:anyURI ;
    dcat:theme legcons:Item .

F2021L00334:365 a legcons:Item,
        owl:Class,
        dcat:Resource ;
    rdfs:label "Item - I365 11 1  Reviewable decisions"@en-AU ;
    dct:isPartOf F2021L00334:364 ;
    dct:isReferencedBy F2021L00334: ;
    rdfs:comment "11 1  Reviewable decisions - Abrievated Graph Key: I365"@en-AU ;
    skos:definition "11 1  Reviewable decisions"@en-AU ;
    skos:narrower F2021L00334:364 ;
    skos:prefLabel "Item I365"@en-AU ;
    dcat:accessURL <https://www.legislation.gov.au/F2021L00334/2023-08-04/2023-08-04/text/original/epub/OEBPS/document_1/document_1.html#_Toc143508012> ;
    dcat:landingPage "https://www.legislation.gov.au/F2021L00334/2023-08-04/2023-08-04/text/original/epub/OEBPS/document_1/document_1.html#_Toc143508012"^^xsd:anyURI ;
    dcat:theme legcons:Item .

F2021L00334:367 a legcons:Item,
        owl:Class,
        dcat:Resource ;
    rdfs:label "Item - I367 11 2  Purpose of this Part"@en-AU ;
    dct:isPartOf F2021L00334:366 ;
    dct:isReferencedBy F2021L00334: ;
    rdfs:comment "11 2  Purpose of this Part - Abrievated Graph Key: I367"@en-AU ;
    skos:definition "11 2  Purpose of this Part"@en-AU ;
    skos:narrower F2021L00334:366 ;
    skos:prefLabel "Item I367"@en-AU ;
    dcat:accessURL <https://www.legislation.gov.au/F2021L00334/2023-08-04/2023-08-04/text/original/epub/OEBPS/document_1/document_1.html#_Toc143508014> ;
    dcat:landingPage "https://www.legislation.gov.au/F2021L00334/2023-08-04/2023-08-04/text/original/epub/OEBPS/document_1/document_1.html#_Toc143508014"^^xsd:anyURI ;
    dcat:theme legcons:Item .

F2021L00334:368 a legcons:Item,
        owl:Class,
        dcat:Resource ;
    rdfs:label "Item - I368 11 3  General requirements for records"@en-AU ;
    dct:isPartOf F2021L00334:366 ;
    dct:isReferencedBy F2021L00334: ;
    rdfs:comment "11 3  General requirements for records - Abrievated Graph Key: I368"@en-AU ;
    skos:definition "11 3  General requirements for records"@en-AU ;
    skos:narrower F2021L00334:366 ;
    skos:prefLabel "Item I368"@en-AU ;
    dcat:accessURL <https://www.legislation.gov.au/F2021L00334/2023-08-04/2023-08-04/text/original/epub/OEBPS/document_1/document_1.html#_Toc143508015> ;
    dcat:landingPage "https://www.legislation.gov.au/F2021L00334/2023-08-04/2023-08-04/text/original/epub/OEBPS/document_1/document_1.html#_Toc143508015"^^xsd:anyURI ;
    dcat:theme legcons:Item .

F2021L00334:369 a legcons:Item,
        owl:Class,
        dcat:Resource ;
    rdfs:label "Item - I369 11 4  Government certificates"@en-AU ;
    dct:isPartOf F2021L00334:366 ;
    dct:isReferencedBy F2021L00334: ;
    rdfs:comment "11 4  Government certificates - Abrievated Graph Key: I369"@en-AU ;
    skos:definition "11 4  Government certificates"@en-AU ;
    skos:narrower F2021L00334:366 ;
    skos:prefLabel "Item I369"@en-AU ;
    dcat:accessURL <https://www.legislation.gov.au/F2021L00334/2023-08-04/2023-08-04/text/original/epub/OEBPS/document_1/document_1.html#_Toc143508016> ;
    dcat:landingPage "https://www.legislation.gov.au/F2021L00334/2023-08-04/2023-08-04/text/original/epub/OEBPS/document_1/document_1.html#_Toc143508016"^^xsd:anyURI ;
    dcat:theme legcons:Item .

F2021L00334:370 a legcons:Item,
        owl:Class,
        dcat:Resource ;
    rdfs:label "Item - I370 11 5  Export permits"@en-AU ;
    dct:isPartOf F2021L00334:366 ;
    dct:isReferencedBy F2021L00334: ;
    rdfs:comment "11 5  Export permits - Abrievated Graph Key: I370"@en-AU ;
    skos:definition "11 5  Export permits"@en-AU ;
    skos:narrower F2021L00334:366 ;
    skos:prefLabel "Item I370"@en-AU ;
    dcat:accessURL <https://www.legislation.gov.au/F2021L00334/2023-08-04/2023-08-04/text/original/epub/OEBPS/document_1/document_1.html#_Toc143508017> ;
    dcat:landingPage "https://www.legislation.gov.au/F2021L00334/2023-08-04/2023-08-04/text/original/epub/OEBPS/document_1/document_1.html#_Toc143508017"^^xsd:anyURI ;
    dcat:theme legcons:Item .

F2021L00334:371 a legcons:Item,
        owl:Class,
        dcat:Resource ;
    rdfs:label "Item - I371 11 6  Records to be retained by exporter"@en-AU ;
    dct:isPartOf F2021L00334:366 ;
    dct:isReferencedBy F2021L00334: ;
    rdfs:comment "11 6  Records to be retained by exporter - Abrievated Graph Key: I371"@en-AU ;
    skos:definition "11 6  Records to be retained by exporter"@en-AU ;
    skos:narrower F2021L00334:366 ;
    skos:prefLabel "Item I371"@en-AU ;
    dcat:accessURL <https://www.legislation.gov.au/F2021L00334/2023-08-04/2023-08-04/text/original/epub/OEBPS/document_1/document_1.html#_Toc143508018> ;
    dcat:landingPage "https://www.legislation.gov.au/F2021L00334/2023-08-04/2023-08-04/text/original/epub/OEBPS/document_1/document_1.html#_Toc143508018"^^xsd:anyURI ;
    dcat:theme legcons:Item .

F2021L00334:372 a legcons:Item,
        owl:Class,
        dcat:Resource ;
    rdfs:label "Item - I372 11 7  Records to be retained by manager of accredited property"@en-AU ;
    dct:isPartOf F2021L00334:366 ;
    dct:isReferencedBy F2021L00334: ;
    rdfs:comment "11 7  Records to be retained by manager of accredited property - Abrievated Graph Key: I372"@en-AU ;
    skos:definition "11 7  Records to be retained by manager of accredited property"@en-AU ;
    skos:narrower F2021L00334:366 ;
    skos:prefLabel "Item I372"@en-AU ;
    dcat:accessURL <https://www.legislation.gov.au/F2021L00334/2023-08-04/2023-08-04/text/original/epub/OEBPS/document_1/document_1.html#_Toc143508019> ;
    dcat:landingPage "https://www.legislation.gov.au/F2021L00334/2023-08-04/2023-08-04/text/original/epub/OEBPS/document_1/document_1.html#_Toc143508019"^^xsd:anyURI ;
    dcat:theme legcons:Item .

F2021L00334:373 a legcons:Item,
        owl:Class,
        dcat:Resource ;
    rdfs:label "Item - I373 11 8  Records to be retained by occupier of registered establishment"@en-AU ;
    dct:isPartOf F2021L00334:366 ;
    dct:isReferencedBy F2021L00334: ;
    rdfs:comment "11 8  Records to be retained by occupier of registered establishment - Abrievated Graph Key: I373"@en-AU ;
    skos:definition "11 8  Records to be retained by occupier of registered establishment"@en-AU ;
    skos:narrower F2021L00334:366 ;
    skos:prefLabel "Item I373"@en-AU ;
    dcat:accessURL <https://www.legislation.gov.au/F2021L00334/2023-08-04/2023-08-04/text/original/epub/OEBPS/document_1/document_1.html#_Toc143508020> ;
    dcat:landingPage "https://www.legislation.gov.au/F2021L00334/2023-08-04/2023-08-04/text/original/epub/OEBPS/document_1/document_1.html#_Toc143508020"^^xsd:anyURI ;
    dcat:theme legcons:Item .

F2021L00334:374 a legcons:Item,
        owl:Class,
        dcat:Resource ;
    rdfs:label "Item - I374 11 9  Records to be retained by holder of approved arrangement"@en-AU ;
    dct:isPartOf F2021L00334:366 ;
    dct:isReferencedBy F2021L00334: ;
    rdfs:comment "11 9  Records to be retained by holder of approved arrangement - Abrievated Graph Key: I374"@en-AU ;
    skos:definition "11 9  Records to be retained by holder of approved arrangement"@en-AU ;
    skos:narrower F2021L00334:366 ;
    skos:prefLabel "Item I374"@en-AU ;
    dcat:accessURL <https://www.legislation.gov.au/F2021L00334/2023-08-04/2023-08-04/text/original/epub/OEBPS/document_1/document_1.html#_Toc143508021> ;
    dcat:landingPage "https://www.legislation.gov.au/F2021L00334/2023-08-04/2023-08-04/text/original/epub/OEBPS/document_1/document_1.html#_Toc143508021"^^xsd:anyURI ;
    dcat:theme legcons:Item .

F2021L00334:375 a legcons:Item,
        owl:Class,
        dcat:Resource ;
    rdfs:label "Item - I375 11 10  Records relating to official marks"@en-AU ;
    dct:isPartOf F2021L00334:366 ;
    dct:isReferencedBy F2021L00334: ;
    rdfs:comment "11 10  Records relating to official marks - Abrievated Graph Key: I375"@en-AU ;
    skos:definition "11 10  Records relating to official marks"@en-AU ;
    skos:narrower F2021L00334:366 ;
    skos:prefLabel "Item I375"@en-AU ;
    dcat:accessURL <https://www.legislation.gov.au/F2021L00334/2023-08-04/2023-08-04/text/original/epub/OEBPS/document_1/document_1.html#_Toc143508022> ;
    dcat:landingPage "https://www.legislation.gov.au/F2021L00334/2023-08-04/2023-08-04/text/original/epub/OEBPS/document_1/document_1.html#_Toc143508022"^^xsd:anyURI ;
    dcat:theme legcons:Item .

F2021L00334:376 a legcons:Item,
        owl:Class,
        dcat:Resource ;
    rdfs:label "Item - I376 11 11  Records relating to official marking devices"@en-AU ;
    dct:isPartOf F2021L00334:366 ;
    dct:isReferencedBy F2021L00334: ;
    rdfs:comment "11 11  Records relating to official marking devices - Abrievated Graph Key: I376"@en-AU ;
    skos:definition "11 11  Records relating to official marking devices"@en-AU ;
    skos:narrower F2021L00334:366 ;
    skos:prefLabel "Item I376"@en-AU ;
    dcat:accessURL <https://www.legislation.gov.au/F2021L00334/2023-08-04/2023-08-04/text/original/epub/OEBPS/document_1/document_1.html#_Toc143508023> ;
    dcat:landingPage "https://www.legislation.gov.au/F2021L00334/2023-08-04/2023-08-04/text/original/epub/OEBPS/document_1/document_1.html#_Toc143508023"^^xsd:anyURI ;
    dcat:theme legcons:Item .

F2021L00334:377 a legcons:Item,
        owl:Class,
        dcat:Resource ;
    rdfs:label "Item - I377 11 12  Records must not be altered or defaced during retention period"@en-AU ;
    dct:isPartOf F2021L00334:366 ;
    dct:isReferencedBy F2021L00334: ;
    rdfs:comment "11 12  Records must not be altered or defaced during retention period - Abrievated Graph Key: I377"@en-AU ;
    skos:definition "11 12  Records must not be altered or defaced during retention period"@en-AU ;
    skos:narrower F2021L00334:366 ;
    skos:prefLabel "Item I377"@en-AU ;
    dcat:accessURL <https://www.legislation.gov.au/F2021L00334/2023-08-04/2023-08-04/text/original/epub/OEBPS/document_1/document_1.html#_Toc143508024> ;
    dcat:landingPage "https://www.legislation.gov.au/F2021L00334/2023-08-04/2023-08-04/text/original/epub/OEBPS/document_1/document_1.html#_Toc143508024"^^xsd:anyURI ;
    dcat:theme legcons:Item .

F2021L00334:379 a legcons:Item,
        owl:Class,
        dcat:Resource ;
    rdfs:label "Item - I379 11 13  Storage of samples"@en-AU ;
    dct:isPartOf F2021L00334:378 ;
    dct:isReferencedBy F2021L00334: ;
    rdfs:comment "11 13  Storage of samples - Abrievated Graph Key: I379"@en-AU ;
    skos:definition "11 13  Storage of samples"@en-AU ;
    skos:narrower F2021L00334:378 ;
    skos:prefLabel "Item I379"@en-AU ;
    dcat:accessURL <https://www.legislation.gov.au/F2021L00334/2023-08-04/2023-08-04/text/original/epub/OEBPS/document_1/document_1.html#_Toc143508026> ;
    dcat:landingPage "https://www.legislation.gov.au/F2021L00334/2023-08-04/2023-08-04/text/original/epub/OEBPS/document_1/document_1.html#_Toc143508026"^^xsd:anyURI ;
    dcat:theme legcons:Item .

F2021L00334:381 a legcons:Item,
        owl:Class,
        dcat:Resource ;
    rdfs:label "Item - I381 11 14  Division of compensation between owners"@en-AU ;
    dct:isPartOf F2021L00334:380 ;
    dct:isReferencedBy F2021L00334: ;
    rdfs:comment "11 14  Division of compensation between owners - Abrievated Graph Key: I381"@en-AU ;
    skos:definition "11 14  Division of compensation between owners"@en-AU ;
    skos:narrower F2021L00334:380 ;
    skos:prefLabel "Item I381"@en-AU ;
    dcat:accessURL <https://www.legislation.gov.au/F2021L00334/2023-08-04/2023-08-04/text/original/epub/OEBPS/document_1/document_1.html#_Toc143508028> ;
    dcat:landingPage "https://www.legislation.gov.au/F2021L00334/2023-08-04/2023-08-04/text/original/epub/OEBPS/document_1/document_1.html#_Toc143508028"^^xsd:anyURI ;
    dcat:theme legcons:Item .

F2021L00334:382 a legcons:Item,
        owl:Class,
        dcat:Resource ;
    rdfs:label "Item - I382 11 15  Amount of compensation"@en-AU ;
    dct:isPartOf F2021L00334:380 ;
    dct:isReferencedBy F2021L00334: ;
    rdfs:comment "11 15  Amount of compensation - Abrievated Graph Key: I382"@en-AU ;
    skos:definition "11 15  Amount of compensation"@en-AU ;
    skos:narrower F2021L00334:380 ;
    skos:prefLabel "Item I382"@en-AU ;
    dcat:accessURL <https://www.legislation.gov.au/F2021L00334/2023-08-04/2023-08-04/text/original/epub/OEBPS/document_1/document_1.html#_Toc143508029> ;
    dcat:landingPage "https://www.legislation.gov.au/F2021L00334/2023-08-04/2023-08-04/text/original/epub/OEBPS/document_1/document_1.html#_Toc143508029"^^xsd:anyURI ;
    dcat:theme legcons:Item .

F2021L00334:384 a legcons:Item,
        owl:Class,
        dcat:Resource ;
    rdfs:label "Item - I384 11 16  Circumstances in which relevant Commonwealth liability of a person is taken to have been paid"@en-AU ;
    dct:isPartOf F2021L00334:383 ;
    dct:isReferencedBy F2021L00334: ;
    rdfs:comment "11 16  Circumstances in which relevant Commonwealth liability of a person is taken to have been paid - Abrievated Graph Key: I384"@en-AU ;
    skos:definition "11 16  Circumstances in which relevant Commonwealth liability of a person is taken to have been paid"@en-AU ;
    skos:narrower F2021L00334:383 ;
    skos:prefLabel "Item I384"@en-AU ;
    dcat:accessURL <https://www.legislation.gov.au/F2021L00334/2023-08-04/2023-08-04/text/original/epub/OEBPS/document_1/document_1.html#_Toc143508031> ;
    dcat:landingPage "https://www.legislation.gov.au/F2021L00334/2023-08-04/2023-08-04/text/original/epub/OEBPS/document_1/document_1.html#_Toc143508031"^^xsd:anyURI ;
    dcat:theme legcons:Item .

F2021L00334:387 a legcons:Item,
        owl:Class,
        dcat:Resource ;
    rdfs:label "Item - I387 12 1  Definitions"@en-AU ;
    dct:isPartOf F2021L00334:386 ;
    dct:isReferencedBy F2021L00334: ;
    rdfs:comment "12 1  Definitions - Abrievated Graph Key: I387"@en-AU ;
    skos:definition "12 1  Definitions"@en-AU ;
    skos:narrower F2021L00334:386 ;
    skos:prefLabel "Item I387"@en-AU ;
    dcat:accessURL <https://www.legislation.gov.au/F2021L00334/2023-08-04/2023-08-04/text/original/epub/OEBPS/document_1/document_1.html#_Toc143508034> ;
    dcat:landingPage "https://www.legislation.gov.au/F2021L00334/2023-08-04/2023-08-04/text/original/epub/OEBPS/document_1/document_1.html#_Toc143508034"^^xsd:anyURI ;
    dcat:theme legcons:Item .

F2021L00334:389 a legcons:Item,
        owl:Class,
        dcat:Resource ;
    rdfs:label "Item - I389 12 2  Allocations of inspection services in effect immediately before commencement time"@en-AU ;
    dct:isPartOf F2021L00334:388 ;
    dct:isReferencedBy F2021L00334: ;
    rdfs:comment "12 2  Allocations of inspection services in effect immediately before commencement time - Abrievated Graph Key: I389"@en-AU ;
    skos:definition "12 2  Allocations of inspection services in effect immediately before commencement time"@en-AU ;
    skos:narrower F2021L00334:388 ;
    skos:prefLabel "Item I389"@en-AU ;
    dcat:accessURL <https://www.legislation.gov.au/F2021L00334/2023-08-04/2023-08-04/text/original/epub/OEBPS/document_1/document_1.html#_Toc143508036> ;
    dcat:landingPage "https://www.legislation.gov.au/F2021L00334/2023-08-04/2023-08-04/text/original/epub/OEBPS/document_1/document_1.html#_Toc143508036"^^xsd:anyURI ;
    dcat:theme legcons:Item .

F2021L00334:39 a legcons:Item,
        owl:Class,
        dcat:Resource ;
    rdfs:label "Item - I39 3 1  Application of this Chapter"@en-AU ;
    dct:isPartOf F2021L00334:38 ;
    dct:isReferencedBy F2021L00334: ;
    rdfs:comment "3 1  Application of this Chapter - Abrievated Graph Key: I39"@en-AU ;
    skos:definition "3 1  Application of this Chapter"@en-AU ;
    skos:narrower F2021L00334:38 ;
    skos:prefLabel "Item I39"@en-AU ;
    dcat:accessURL <https://www.legislation.gov.au/F2021L00334/2023-08-04/2023-08-04/text/original/epub/OEBPS/document_1/document_1.html#_Toc143507686> ;
    dcat:landingPage "https://www.legislation.gov.au/F2021L00334/2023-08-04/2023-08-04/text/original/epub/OEBPS/document_1/document_1.html#_Toc143507686"^^xsd:anyURI ;
    dcat:theme legcons:Item .

F2021L00334:390 a legcons:Item,
        owl:Class,
        dcat:Resource ;
    rdfs:label "Item - I390 12 3  Application for inspection services not decided or notice of decision not given before commencement time"@en-AU ;
    dct:isPartOf F2021L00334:388 ;
    dct:isReferencedBy F2021L00334: ;
    rdfs:comment "12 3  Application for inspection services not decided or notice of decision not given before commencement time - Abrievated Graph Key: I390"@en-AU ;
    skos:definition "12 3  Application for inspection services not decided or notice of decision not given before commencement time"@en-AU ;
    skos:narrower F2021L00334:388 ;
    skos:prefLabel "Item I390"@en-AU ;
    dcat:accessURL <https://www.legislation.gov.au/F2021L00334/2023-08-04/2023-08-04/text/original/epub/OEBPS/document_1/document_1.html#_Toc143508037> ;
    dcat:landingPage "https://www.legislation.gov.au/F2021L00334/2023-08-04/2023-08-04/text/original/epub/OEBPS/document_1/document_1.html#_Toc143508037"^^xsd:anyURI ;
    dcat:theme legcons:Item .

F2021L00334:391 a legcons:Item,
        owl:Class,
        dcat:Resource ;
    rdfs:label "Item - I391 12 4  Notice of preliminary determination of allocation given before commencement time"@en-AU ;
    dct:isPartOf F2021L00334:388 ;
    dct:isReferencedBy F2021L00334: ;
    rdfs:comment "12 4  Notice of preliminary determination of allocation given before commencement time - Abrievated Graph Key: I391"@en-AU ;
    skos:definition "12 4  Notice of preliminary determination of allocation given before commencement time"@en-AU ;
    skos:narrower F2021L00334:388 ;
    skos:prefLabel "Item I391"@en-AU ;
    dcat:accessURL <https://www.legislation.gov.au/F2021L00334/2023-08-04/2023-08-04/text/original/epub/OEBPS/document_1/document_1.html#_Toc143508038> ;
    dcat:landingPage "https://www.legislation.gov.au/F2021L00334/2023-08-04/2023-08-04/text/original/epub/OEBPS/document_1/document_1.html#_Toc143508038"^^xsd:anyURI ;
    dcat:theme legcons:Item .

F2021L00334:392 a legcons:Item,
        owl:Class,
        dcat:Resource ;
    rdfs:label "Item - I392 12 5  Preliminary determination of allocation agreed before commencement time"@en-AU ;
    dct:isPartOf F2021L00334:388 ;
    dct:isReferencedBy F2021L00334: ;
    rdfs:comment "12 5  Preliminary determination of allocation agreed before commencement time - Abrievated Graph Key: I392"@en-AU ;
    skos:definition "12 5  Preliminary determination of allocation agreed before commencement time"@en-AU ;
    skos:narrower F2021L00334:388 ;
    skos:prefLabel "Item I392"@en-AU ;
    dcat:accessURL <https://www.legislation.gov.au/F2021L00334/2023-08-04/2023-08-04/text/original/epub/OEBPS/document_1/document_1.html#_Toc143508039> ;
    dcat:landingPage "https://www.legislation.gov.au/F2021L00334/2023-08-04/2023-08-04/text/original/epub/OEBPS/document_1/document_1.html#_Toc143508039"^^xsd:anyURI ;
    dcat:theme legcons:Item .

F2021L00334:393 a legcons:Item,
        owl:Class,
        dcat:Resource ;
    rdfs:label "Item - I393 12 6  Revised determination made but notice not given before commencement time"@en-AU ;
    dct:isPartOf F2021L00334:388 ;
    dct:isReferencedBy F2021L00334: ;
    rdfs:comment "12 6  Revised determination made but notice not given before commencement time - Abrievated Graph Key: I393"@en-AU ;
    skos:definition "12 6  Revised determination made but notice not given before commencement time"@en-AU ;
    skos:narrower F2021L00334:388 ;
    skos:prefLabel "Item I393"@en-AU ;
    dcat:accessURL <https://www.legislation.gov.au/F2021L00334/2023-08-04/2023-08-04/text/original/epub/OEBPS/document_1/document_1.html#_Toc143508040> ;
    dcat:landingPage "https://www.legislation.gov.au/F2021L00334/2023-08-04/2023-08-04/text/original/epub/OEBPS/document_1/document_1.html#_Toc143508040"^^xsd:anyURI ;
    dcat:theme legcons:Item .

F2021L00334:394 a legcons:Item,
        owl:Class,
        dcat:Resource ;
    rdfs:label "Item - I394 12 7  Notice of revised determination of inspection services given before commencement time"@en-AU ;
    dct:isPartOf F2021L00334:388 ;
    dct:isReferencedBy F2021L00334: ;
    rdfs:comment "12 7  Notice of revised determination of inspection services given before commencement time - Abrievated Graph Key: I394"@en-AU ;
    skos:definition "12 7  Notice of revised determination of inspection services given before commencement time"@en-AU ;
    skos:narrower F2021L00334:388 ;
    skos:prefLabel "Item I394"@en-AU ;
    dcat:accessURL <https://www.legislation.gov.au/F2021L00334/2023-08-04/2023-08-04/text/original/epub/OEBPS/document_1/document_1.html#_Toc143508041> ;
    dcat:landingPage "https://www.legislation.gov.au/F2021L00334/2023-08-04/2023-08-04/text/original/epub/OEBPS/document_1/document_1.html#_Toc143508041"^^xsd:anyURI ;
    dcat:theme legcons:Item .

F2021L00334:395 a legcons:Item,
        owl:Class,
        dcat:Resource ;
    rdfs:label "Item - I395 12 8  Revised determination of allocation agreed before commencement time"@en-AU ;
    dct:isPartOf F2021L00334:388 ;
    dct:isReferencedBy F2021L00334: ;
    rdfs:comment "12 8  Revised determination of allocation agreed before commencement time - Abrievated Graph Key: I395"@en-AU ;
    skos:definition "12 8  Revised determination of allocation agreed before commencement time"@en-AU ;
    skos:narrower F2021L00334:388 ;
    skos:prefLabel "Item I395"@en-AU ;
    dcat:accessURL <https://www.legislation.gov.au/F2021L00334/2023-08-04/2023-08-04/text/original/epub/OEBPS/document_1/document_1.html#_Toc143508042> ;
    dcat:landingPage "https://www.legislation.gov.au/F2021L00334/2023-08-04/2023-08-04/text/original/epub/OEBPS/document_1/document_1.html#_Toc143508042"^^xsd:anyURI ;
    dcat:theme legcons:Item .

F2021L00334:396 a legcons:Item,
        owl:Class,
        dcat:Resource ;
    rdfs:label "Item - I396 12 9  Application for review committee made but committee not established before commencement time"@en-AU ;
    dct:isPartOf F2021L00334:388 ;
    dct:isReferencedBy F2021L00334: ;
    rdfs:comment "12 9  Application for review committee made but committee not established before commencement time - Abrievated Graph Key: I396"@en-AU ;
    skos:definition "12 9  Application for review committee made but committee not established before commencement time"@en-AU ;
    skos:narrower F2021L00334:388 ;
    skos:prefLabel "Item I396"@en-AU ;
    dcat:accessURL <https://www.legislation.gov.au/F2021L00334/2023-08-04/2023-08-04/text/original/epub/OEBPS/document_1/document_1.html#_Toc143508043> ;
    dcat:landingPage "https://www.legislation.gov.au/F2021L00334/2023-08-04/2023-08-04/text/original/epub/OEBPS/document_1/document_1.html#_Toc143508043"^^xsd:anyURI ;
    dcat:theme legcons:Item .

F2021L00334:397 a legcons:Item,
        owl:Class,
        dcat:Resource ;
    rdfs:label "Item - I397 12 10  Committee review in progress before commencement time"@en-AU ;
    dct:isPartOf F2021L00334:388 ;
    dct:isReferencedBy F2021L00334: ;
    rdfs:comment "12 10  Committee review in progress before commencement time - Abrievated Graph Key: I397"@en-AU ;
    skos:definition "12 10  Committee review in progress before commencement time"@en-AU ;
    skos:narrower F2021L00334:388 ;
    skos:prefLabel "Item I397"@en-AU ;
    dcat:accessURL <https://www.legislation.gov.au/F2021L00334/2023-08-04/2023-08-04/text/original/epub/OEBPS/document_1/document_1.html#_Toc143508044> ;
    dcat:landingPage "https://www.legislation.gov.au/F2021L00334/2023-08-04/2023-08-04/text/original/epub/OEBPS/document_1/document_1.html#_Toc143508044"^^xsd:anyURI ;
    dcat:theme legcons:Item .

F2021L00334:398 a legcons:Item,
        owl:Class,
        dcat:Resource ;
    rdfs:label "Item - I398 12 11  Determination reconsidered but notice not given before commencement time"@en-AU ;
    dct:isPartOf F2021L00334:388 ;
    dct:isReferencedBy F2021L00334: ;
    rdfs:comment "12 11  Determination reconsidered but notice not given before commencement time - Abrievated Graph Key: I398"@en-AU ;
    skos:definition "12 11  Determination reconsidered but notice not given before commencement time"@en-AU ;
    skos:narrower F2021L00334:388 ;
    skos:prefLabel "Item I398"@en-AU ;
    dcat:accessURL <https://www.legislation.gov.au/F2021L00334/2023-08-04/2023-08-04/text/original/epub/OEBPS/document_1/document_1.html#_Toc143508045> ;
    dcat:landingPage "https://www.legislation.gov.au/F2021L00334/2023-08-04/2023-08-04/text/original/epub/OEBPS/document_1/document_1.html#_Toc143508045"^^xsd:anyURI ;
    dcat:theme legcons:Item .

F2021L00334:399 a legcons:Item,
        owl:Class,
        dcat:Resource ;
    rdfs:label "Item - I399 12 12  Application to alter inspection services not decided before commencement time"@en-AU ;
    dct:isPartOf F2021L00334:388 ;
    dct:isReferencedBy F2021L00334: ;
    rdfs:comment "12 12  Application to alter inspection services not decided before commencement time - Abrievated Graph Key: I399"@en-AU ;
    skos:definition "12 12  Application to alter inspection services not decided before commencement time"@en-AU ;
    skos:narrower F2021L00334:388 ;
    skos:prefLabel "Item I399"@en-AU ;
    dcat:accessURL <https://www.legislation.gov.au/F2021L00334/2023-08-04/2023-08-04/text/original/epub/OEBPS/document_1/document_1.html#_Toc143508046> ;
    dcat:landingPage "https://www.legislation.gov.au/F2021L00334/2023-08-04/2023-08-04/text/original/epub/OEBPS/document_1/document_1.html#_Toc143508046"^^xsd:anyURI ;
    dcat:theme legcons:Item .

F2021L00334:4 a legcons:Item,
        owl:Class,
        dcat:Resource ;
    rdfs:label "Item - I4 1 3  Authority"@en-AU ;
    dct:isPartOf F2021L00334:1 ;
    dct:isReferencedBy F2021L00334: ;
    rdfs:comment "1 3  Authority - Abrievated Graph Key: I4"@en-AU ;
    skos:definition "1 3  Authority"@en-AU ;
    skos:narrower F2021L00334:1 ;
    skos:prefLabel "Item I4"@en-AU ;
    dcat:accessURL <https://www.legislation.gov.au/F2021L00334/2023-08-04/2023-08-04/text/original/epub/OEBPS/document_1/document_1.html#_Toc143507651> ;
    dcat:landingPage "https://www.legislation.gov.au/F2021L00334/2023-08-04/2023-08-04/text/original/epub/OEBPS/document_1/document_1.html#_Toc143507651"^^xsd:anyURI ;
    dcat:theme legcons:Item .

F2021L00334:40 a legcons:Item,
        owl:Class,
        dcat:Resource ;
    rdfs:label "Item - I40 3 2  When an animal is taken to have been treated with an HGP"@en-AU ;
    dct:isPartOf F2021L00334:38 ;
    dct:isReferencedBy F2021L00334: ;
    rdfs:comment "3 2  When an animal is taken to have been treated with an HGP - Abrievated Graph Key: I40"@en-AU ;
    skos:definition "3 2  When an animal is taken to have been treated with an HGP"@en-AU ;
    skos:narrower F2021L00334:38 ;
    skos:prefLabel "Item I40"@en-AU ;
    dcat:accessURL <https://www.legislation.gov.au/F2021L00334/2023-08-04/2023-08-04/text/original/epub/OEBPS/document_1/document_1.html#_Toc143507687> ;
    dcat:landingPage "https://www.legislation.gov.au/F2021L00334/2023-08-04/2023-08-04/text/original/epub/OEBPS/document_1/document_1.html#_Toc143507687"^^xsd:anyURI ;
    dcat:theme legcons:Item .

F2021L00334:400 a legcons:Item,
        owl:Class,
        dcat:Resource ;
    rdfs:label "Item - I400 12 13  Application for additional inspection services not decided before commencement time"@en-AU ;
    dct:isPartOf F2021L00334:388 ;
    dct:isReferencedBy F2021L00334: ;
    rdfs:comment "12 13  Application for additional inspection services not decided before commencement time - Abrievated Graph Key: I400"@en-AU ;
    skos:definition "12 13  Application for additional inspection services not decided before commencement time"@en-AU ;
    skos:narrower F2021L00334:388 ;
    skos:prefLabel "Item I400"@en-AU ;
    dcat:accessURL <https://www.legislation.gov.au/F2021L00334/2023-08-04/2023-08-04/text/original/epub/OEBPS/document_1/document_1.html#_Toc143508047> ;
    dcat:landingPage "https://www.legislation.gov.au/F2021L00334/2023-08-04/2023-08-04/text/original/epub/OEBPS/document_1/document_1.html#_Toc143508047"^^xsd:anyURI ;
    dcat:theme legcons:Item .

F2021L00334:401 a legcons:Item,
        owl:Class,
        dcat:Resource ;
    rdfs:label "Item - I401 12 14  Notice of termination of additional inspection services given before commencement time"@en-AU ;
    dct:isPartOf F2021L00334:388 ;
    dct:isReferencedBy F2021L00334: ;
    rdfs:comment "12 14  Notice of termination of additional inspection services given before commencement time - Abrievated Graph Key: I401"@en-AU ;
    skos:definition "12 14  Notice of termination of additional inspection services given before commencement time"@en-AU ;
    skos:narrower F2021L00334:388 ;
    skos:prefLabel "Item I401"@en-AU ;
    dcat:accessURL <https://www.legislation.gov.au/F2021L00334/2023-08-04/2023-08-04/text/original/epub/OEBPS/document_1/document_1.html#_Toc143508048> ;
    dcat:landingPage "https://www.legislation.gov.au/F2021L00334/2023-08-04/2023-08-04/text/original/epub/OEBPS/document_1/document_1.html#_Toc143508048"^^xsd:anyURI ;
    dcat:theme legcons:Item .

F2021L00334:402 a legcons:Item,
        owl:Class,
        dcat:Resource ;
    rdfs:label "Item - I402 12 15  Notice of shutdown given before commencement time"@en-AU ;
    dct:isPartOf F2021L00334:388 ;
    dct:isReferencedBy F2021L00334: ;
    rdfs:comment "12 15  Notice of shutdown given before commencement time - Abrievated Graph Key: I402"@en-AU ;
    skos:definition "12 15  Notice of shutdown given before commencement time"@en-AU ;
    skos:narrower F2021L00334:388 ;
    skos:prefLabel "Item I402"@en-AU ;
    dcat:accessURL <https://www.legislation.gov.au/F2021L00334/2023-08-04/2023-08-04/text/original/epub/OEBPS/document_1/document_1.html#_Toc143508049> ;
    dcat:landingPage "https://www.legislation.gov.au/F2021L00334/2023-08-04/2023-08-04/text/original/epub/OEBPS/document_1/document_1.html#_Toc143508049"^^xsd:anyURI ;
    dcat:theme legcons:Item .

F2021L00334:403 a legcons:Item,
        owl:Class,
        dcat:Resource ;
    rdfs:label "Item - I403 12 16  Variation of allocation for change of circumstance not advised before commencement time"@en-AU ;
    dct:isPartOf F2021L00334:388 ;
    dct:isReferencedBy F2021L00334: ;
    rdfs:comment "12 16  Variation of allocation for change of circumstance not advised before commencement time - Abrievated Graph Key: I403"@en-AU ;
    skos:definition "12 16  Variation of allocation for change of circumstance not advised before commencement time"@en-AU ;
    skos:narrower F2021L00334:388 ;
    skos:prefLabel "Item I403"@en-AU ;
    dcat:accessURL <https://www.legislation.gov.au/F2021L00334/2023-08-04/2023-08-04/text/original/epub/OEBPS/document_1/document_1.html#_Toc143508050> ;
    dcat:landingPage "https://www.legislation.gov.au/F2021L00334/2023-08-04/2023-08-04/text/original/epub/OEBPS/document_1/document_1.html#_Toc143508050"^^xsd:anyURI ;
    dcat:theme legcons:Item .

F2021L00334:404 a legcons:Item,
        owl:Class,
        dcat:Resource ;
    rdfs:label "Item - I404 12 17  Disputed allocation not decided before commencement time"@en-AU ;
    dct:isPartOf F2021L00334:388 ;
    dct:isReferencedBy F2021L00334: ;
    rdfs:comment "12 17  Disputed allocation not decided before commencement time - Abrievated Graph Key: I404"@en-AU ;
    skos:definition "12 17  Disputed allocation not decided before commencement time"@en-AU ;
    skos:narrower F2021L00334:388 ;
    skos:prefLabel "Item I404"@en-AU ;
    dcat:accessURL <https://www.legislation.gov.au/F2021L00334/2023-08-04/2023-08-04/text/original/epub/OEBPS/document_1/document_1.html#_Toc143508051> ;
    dcat:landingPage "https://www.legislation.gov.au/F2021L00334/2023-08-04/2023-08-04/text/original/epub/OEBPS/document_1/document_1.html#_Toc143508051"^^xsd:anyURI ;
    dcat:theme legcons:Item .

F2021L00334:405 a legcons:Item,
        owl:Class,
        dcat:Resource ;
    rdfs:label "Item - I405 12 18  Notice of reconsideration of disputed allocation not given before commencement time"@en-AU ;
    dct:isPartOf F2021L00334:388 ;
    dct:isReferencedBy F2021L00334: ;
    rdfs:comment "12 18  Notice of reconsideration of disputed allocation not given before commencement time - Abrievated Graph Key: I405"@en-AU ;
    skos:definition "12 18  Notice of reconsideration of disputed allocation not given before commencement time"@en-AU ;
    skos:narrower F2021L00334:388 ;
    skos:prefLabel "Item I405"@en-AU ;
    dcat:accessURL <https://www.legislation.gov.au/F2021L00334/2023-08-04/2023-08-04/text/original/epub/OEBPS/document_1/document_1.html#_Toc143508052> ;
    dcat:landingPage "https://www.legislation.gov.au/F2021L00334/2023-08-04/2023-08-04/text/original/epub/OEBPS/document_1/document_1.html#_Toc143508052"^^xsd:anyURI ;
    dcat:theme legcons:Item .

F2021L00334:407 a legcons:Item,
        owl:Class,
        dcat:Resource ;
    rdfs:label "Item - I407 12 19  Information and declarations given before commencement time"@en-AU ;
    dct:isPartOf F2021L00334:406 ;
    dct:isReferencedBy F2021L00334: ;
    rdfs:comment "12 19  Information and declarations given before commencement time - Abrievated Graph Key: I407"@en-AU ;
    skos:definition "12 19  Information and declarations given before commencement time"@en-AU ;
    skos:narrower F2021L00334:406 ;
    skos:prefLabel "Item I407"@en-AU ;
    dcat:accessURL <https://www.legislation.gov.au/F2021L00334/2023-08-04/2023-08-04/text/original/epub/OEBPS/document_1/document_1.html#_Toc143508054> ;
    dcat:landingPage "https://www.legislation.gov.au/F2021L00334/2023-08-04/2023-08-04/text/original/epub/OEBPS/document_1/document_1.html#_Toc143508054"^^xsd:anyURI ;
    dcat:theme legcons:Item .

F2021L00334:410 a legcons:Item,
        owl:Class,
        dcat:Resource ;
    rdfs:label "Item - I410 12 20  Request for translation not complied with before commencement time"@en-AU ;
    dct:isPartOf F2021L00334:409 ;
    dct:isReferencedBy F2021L00334: ;
    rdfs:comment "12 20  Request for translation not complied with before commencement time - Abrievated Graph Key: I410"@en-AU ;
    skos:definition "12 20  Request for translation not complied with before commencement time"@en-AU ;
    skos:narrower F2021L00334:409 ;
    skos:prefLabel "Item I410"@en-AU ;
    dcat:accessURL <https://www.legislation.gov.au/F2021L00334/2023-08-04/2023-08-04/text/original/epub/OEBPS/document_1/document_1.html#_Toc143508057> ;
    dcat:landingPage "https://www.legislation.gov.au/F2021L00334/2023-08-04/2023-08-04/text/original/epub/OEBPS/document_1/document_1.html#_Toc143508057"^^xsd:anyURI ;
    dcat:theme legcons:Item .

F2021L00334:412 a legcons:Item,
        owl:Class,
        dcat:Resource ;
    rdfs:label "Item - I412 12 21  Person approved before commencement time to manufacture an official mark"@en-AU ;
    dct:isPartOf F2021L00334:411 ;
    dct:isReferencedBy F2021L00334: ;
    rdfs:comment "12 21  Person approved before commencement time to manufacture an official mark - Abrievated Graph Key: I412"@en-AU ;
    skos:definition "12 21  Person approved before commencement time to manufacture an official mark"@en-AU ;
    skos:narrower F2021L00334:411 ;
    skos:prefLabel "Item I412"@en-AU ;
    dcat:accessURL <https://www.legislation.gov.au/F2021L00334/2023-08-04/2023-08-04/text/original/epub/OEBPS/document_1/document_1.html#_Toc143508059> ;
    dcat:landingPage "https://www.legislation.gov.au/F2021L00334/2023-08-04/2023-08-04/text/original/epub/OEBPS/document_1/document_1.html#_Toc143508059"^^xsd:anyURI ;
    dcat:theme legcons:Item .

F2021L00334:413 a legcons:Item,
        owl:Class,
        dcat:Resource ;
    rdfs:label "Item - I413 12 22  Person approved before commencement time to possess an official mark"@en-AU ;
    dct:isPartOf F2021L00334:411 ;
    dct:isReferencedBy F2021L00334: ;
    rdfs:comment "12 22  Person approved before commencement time to possess an official mark - Abrievated Graph Key: I413"@en-AU ;
    skos:definition "12 22  Person approved before commencement time to possess an official mark"@en-AU ;
    skos:narrower F2021L00334:411 ;
    skos:prefLabel "Item I413"@en-AU ;
    dcat:accessURL <https://www.legislation.gov.au/F2021L00334/2023-08-04/2023-08-04/text/original/epub/OEBPS/document_1/document_1.html#_Toc143508060> ;
    dcat:landingPage "https://www.legislation.gov.au/F2021L00334/2023-08-04/2023-08-04/text/original/epub/OEBPS/document_1/document_1.html#_Toc143508060"^^xsd:anyURI ;
    dcat:theme legcons:Item .

F2021L00334:414 a legcons:Item,
        owl:Class,
        dcat:Resource ;
    rdfs:label "Item - I414 12 23  Person approved before commencement time to apply an official mark"@en-AU ;
    dct:isPartOf F2021L00334:411 ;
    dct:isReferencedBy F2021L00334: ;
    rdfs:comment "12 23  Person approved before commencement time to apply an official mark - Abrievated Graph Key: I414"@en-AU ;
    skos:definition "12 23  Person approved before commencement time to apply an official mark"@en-AU ;
    skos:narrower F2021L00334:411 ;
    skos:prefLabel "Item I414"@en-AU ;
    dcat:accessURL <https://www.legislation.gov.au/F2021L00334/2023-08-04/2023-08-04/text/original/epub/OEBPS/document_1/document_1.html#_Toc143508061> ;
    dcat:landingPage "https://www.legislation.gov.au/F2021L00334/2023-08-04/2023-08-04/text/original/epub/OEBPS/document_1/document_1.html#_Toc143508061"^^xsd:anyURI ;
    dcat:theme legcons:Item .

F2021L00334:416 a legcons:Item,
        owl:Class,
        dcat:Resource ;
    rdfs:label "Item - I416 12 24  Person approved before commencement time to manufacture an official marking device"@en-AU ;
    dct:isPartOf F2021L00334:415 ;
    dct:isReferencedBy F2021L00334: ;
    rdfs:comment "12 24  Person approved before commencement time to manufacture an official marking device - Abrievated Graph Key: I416"@en-AU ;
    skos:definition "12 24  Person approved before commencement time to manufacture an official marking device"@en-AU ;
    skos:narrower F2021L00334:415 ;
    skos:prefLabel "Item I416"@en-AU ;
    dcat:accessURL <https://www.legislation.gov.au/F2021L00334/2023-08-04/2023-08-04/text/original/epub/OEBPS/document_1/document_1.html#_Toc143508063> ;
    dcat:landingPage "https://www.legislation.gov.au/F2021L00334/2023-08-04/2023-08-04/text/original/epub/OEBPS/document_1/document_1.html#_Toc143508063"^^xsd:anyURI ;
    dcat:theme legcons:Item .

F2021L00334:417 a legcons:Item,
        owl:Class,
        dcat:Resource ;
    rdfs:label "Item - I417 12 25  Person approved before commencement time to possess an official marking device"@en-AU ;
    dct:isPartOf F2021L00334:415 ;
    dct:isReferencedBy F2021L00334: ;
    rdfs:comment "12 25  Person approved before commencement time to possess an official marking device - Abrievated Graph Key: I417"@en-AU ;
    skos:definition "12 25  Person approved before commencement time to possess an official marking device"@en-AU ;
    skos:narrower F2021L00334:415 ;
    skos:prefLabel "Item I417"@en-AU ;
    dcat:accessURL <https://www.legislation.gov.au/F2021L00334/2023-08-04/2023-08-04/text/original/epub/OEBPS/document_1/document_1.html#_Toc143508064> ;
    dcat:landingPage "https://www.legislation.gov.au/F2021L00334/2023-08-04/2023-08-04/text/original/epub/OEBPS/document_1/document_1.html#_Toc143508064"^^xsd:anyURI ;
    dcat:theme legcons:Item .

F2021L00334:420 a legcons:Item,
        owl:Class,
        dcat:Resource ;
    rdfs:label "Item - I420 12 26  Application for approval as auditor not decided or notice of decision not given before commencement time"@en-AU ;
    dct:isPartOf F2021L00334:419 ;
    dct:isReferencedBy F2021L00334: ;
    rdfs:comment "12 26  Application for approval as auditor not decided or notice of decision not given before commencement time - Abrievated Graph Key: I420"@en-AU ;
    skos:definition "12 26  Application for approval as auditor not decided or notice of decision not given before commencement time"@en-AU ;
    skos:narrower F2021L00334:419 ;
    skos:prefLabel "Item I420"@en-AU ;
    dcat:accessURL <https://www.legislation.gov.au/F2021L00334/2023-08-04/2023-08-04/text/original/epub/OEBPS/document_1/document_1.html#_Toc143508067> ;
    dcat:landingPage "https://www.legislation.gov.au/F2021L00334/2023-08-04/2023-08-04/text/original/epub/OEBPS/document_1/document_1.html#_Toc143508067"^^xsd:anyURI ;
    dcat:theme legcons:Item .

F2021L00334:421 a legcons:Item,
        owl:Class,
        dcat:Resource ;
    rdfs:label "Item - I421 12 27  Request for further information not complied with before commencement time"@en-AU ;
    dct:isPartOf F2021L00334:419 ;
    dct:isReferencedBy F2021L00334: ;
    rdfs:comment "12 27  Request for further information not complied with before commencement time - Abrievated Graph Key: I421"@en-AU ;
    skos:definition "12 27  Request for further information not complied with before commencement time"@en-AU ;
    skos:narrower F2021L00334:419 ;
    skos:prefLabel "Item I421"@en-AU ;
    dcat:accessURL <https://www.legislation.gov.au/F2021L00334/2023-08-04/2023-08-04/text/original/epub/OEBPS/document_1/document_1.html#_Toc143508068> ;
    dcat:landingPage "https://www.legislation.gov.au/F2021L00334/2023-08-04/2023-08-04/text/original/epub/OEBPS/document_1/document_1.html#_Toc143508068"^^xsd:anyURI ;
    dcat:theme legcons:Item .

F2021L00334:422 a legcons:Item,
        owl:Class,
        dcat:Resource ;
    rdfs:label "Item - I422 12 28  Decision to revoke approval as auditor decided but notice not given before commencement time"@en-AU ;
    dct:isPartOf F2021L00334:419 ;
    dct:isReferencedBy F2021L00334: ;
    rdfs:comment "12 28  Decision to revoke approval as auditor decided but notice not given before commencement time - Abrievated Graph Key: I422"@en-AU ;
    skos:definition "12 28  Decision to revoke approval as auditor decided but notice not given before commencement time"@en-AU ;
    skos:narrower F2021L00334:419 ;
    skos:prefLabel "Item I422"@en-AU ;
    dcat:accessURL <https://www.legislation.gov.au/F2021L00334/2023-08-04/2023-08-04/text/original/epub/OEBPS/document_1/document_1.html#_Toc143508069> ;
    dcat:landingPage "https://www.legislation.gov.au/F2021L00334/2023-08-04/2023-08-04/text/original/epub/OEBPS/document_1/document_1.html#_Toc143508069"^^xsd:anyURI ;
    dcat:theme legcons:Item .

F2021L00334:424 a legcons:Item,
        owl:Class,
        dcat:Resource ;
    rdfs:label "Item - I424 12 29  Written advice about admission of animal for slaughter given but animal not admitted before commencement time"@en-AU ;
    dct:isPartOf F2021L00334:423 ;
    dct:isReferencedBy F2021L00334: ;
    rdfs:comment "12 29  Written advice about admission of animal for slaughter given but animal not admitted before commencement time - Abrievated Graph Key: I424"@en-AU ;
    skos:definition "12 29  Written advice about admission of animal for slaughter given but animal not admitted before commencement time"@en-AU ;
    skos:narrower F2021L00334:423 ;
    skos:prefLabel "Item I424"@en-AU ;
    dcat:accessURL <https://www.legislation.gov.au/F2021L00334/2023-08-04/2023-08-04/text/original/epub/OEBPS/document_1/document_1.html#_Toc143508071> ;
    dcat:landingPage "https://www.legislation.gov.au/F2021L00334/2023-08-04/2023-08-04/text/original/epub/OEBPS/document_1/document_1.html#_Toc143508071"^^xsd:anyURI ;
    dcat:theme legcons:Item .

F2021L00334:425 a legcons:Item,
        owl:Class,
        dcat:Resource ;
    rdfs:label "Item - I425 12 30  Decision or disposition applied but not complied with before commencement time"@en-AU ;
    dct:isPartOf F2021L00334:423 ;
    dct:isReferencedBy F2021L00334: ;
    rdfs:comment "12 30  Decision or disposition applied but not complied with before commencement time - Abrievated Graph Key: I425"@en-AU ;
    skos:definition "12 30  Decision or disposition applied but not complied with before commencement time"@en-AU ;
    skos:narrower F2021L00334:423 ;
    skos:prefLabel "Item I425"@en-AU ;
    dcat:accessURL <https://www.legislation.gov.au/F2021L00334/2023-08-04/2023-08-04/text/original/epub/OEBPS/document_1/document_1.html#_Toc143508072> ;
    dcat:landingPage "https://www.legislation.gov.au/F2021L00334/2023-08-04/2023-08-04/text/original/epub/OEBPS/document_1/document_1.html#_Toc143508072"^^xsd:anyURI ;
    dcat:theme legcons:Item .

F2021L00334:426 a legcons:Item,
        owl:Class,
        dcat:Resource ;
    rdfs:label "Item - I426 12 31  Certificate of condemnation requested but not given before commencement time"@en-AU ;
    dct:isPartOf F2021L00334:423 ;
    dct:isReferencedBy F2021L00334: ;
    rdfs:comment "12 31  Certificate of condemnation requested but not given before commencement time - Abrievated Graph Key: I426"@en-AU ;
    skos:definition "12 31  Certificate of condemnation requested but not given before commencement time"@en-AU ;
    skos:narrower F2021L00334:423 ;
    skos:prefLabel "Item I426"@en-AU ;
    dcat:accessURL <https://www.legislation.gov.au/F2021L00334/2023-08-04/2023-08-04/text/original/epub/OEBPS/document_1/document_1.html#_Toc143508073> ;
    dcat:landingPage "https://www.legislation.gov.au/F2021L00334/2023-08-04/2023-08-04/text/original/epub/OEBPS/document_1/document_1.html#_Toc143508073"^^xsd:anyURI ;
    dcat:theme legcons:Item .

F2021L00334:428 a legcons:Item,
        owl:Class,
        dcat:Resource ;
    rdfs:label "Item - I428 Endnote 1 About the endnotes"@en-AU ;
    dct:isPartOf F2021L00334:427 ;
    dct:isReferencedBy F2021L00334: ;
    rdfs:comment "Endnote 1 About the endnotes - Abrievated Graph Key: I428"@en-AU ;
    skos:definition "Endnote 1 About the endnotes"@en-AU ;
    skos:narrower F2021L00334:427 ;
    skos:prefLabel "Item I428"@en-AU ;
    dcat:accessURL <https://www.legislation.gov.au/F2021L00334/2023-08-04/2023-08-04/text/original/epub/OEBPS/document_1/document_1.html#_Toc143508075> ;
    dcat:landingPage "https://www.legislation.gov.au/F2021L00334/2023-08-04/2023-08-04/text/original/epub/OEBPS/document_1/document_1.html#_Toc143508075"^^xsd:anyURI ;
    dcat:theme legcons:Item .

F2021L00334:429 a legcons:Item,
        owl:Class,
        dcat:Resource ;
    rdfs:label "Item - I429 Endnote 2 Abbreviation key"@en-AU ;
    dct:isPartOf F2021L00334:427 ;
    dct:isReferencedBy F2021L00334: ;
    rdfs:comment "Endnote 2 Abbreviation key - Abrievated Graph Key: I429"@en-AU ;
    skos:definition "Endnote 2 Abbreviation key"@en-AU ;
    skos:narrower F2021L00334:427 ;
    skos:prefLabel "Item I429"@en-AU ;
    dcat:accessURL <https://www.legislation.gov.au/F2021L00334/2023-08-04/2023-08-04/text/original/epub/OEBPS/document_1/document_1.html#_Toc143508076> ;
    dcat:landingPage "https://www.legislation.gov.au/F2021L00334/2023-08-04/2023-08-04/text/original/epub/OEBPS/document_1/document_1.html#_Toc143508076"^^xsd:anyURI ;
    dcat:theme legcons:Item .

F2021L00334:43 a legcons:Item,
        owl:Class,
        dcat:Resource ;
    rdfs:label "Item - I43 3 3  Purpose of this Division"@en-AU ;
    dct:isPartOf F2021L00334:42 ;
    dct:isReferencedBy F2021L00334: ;
    rdfs:comment "3 3  Purpose of this Division - Abrievated Graph Key: I43"@en-AU ;
    skos:definition "3 3  Purpose of this Division"@en-AU ;
    skos:narrower F2021L00334:42 ;
    skos:prefLabel "Item I43"@en-AU ;
    dcat:accessURL <https://www.legislation.gov.au/F2021L00334/2023-08-04/2023-08-04/text/original/epub/OEBPS/document_1/document_1.html#_Toc143507690> ;
    dcat:landingPage "https://www.legislation.gov.au/F2021L00334/2023-08-04/2023-08-04/text/original/epub/OEBPS/document_1/document_1.html#_Toc143507690"^^xsd:anyURI ;
    dcat:theme legcons:Item .

F2021L00334:430 a legcons:Item,
        owl:Class,
        dcat:Resource ;
    rdfs:label "Item - I430 Endnote 3 Legislation history"@en-AU ;
    dct:isPartOf F2021L00334:427 ;
    dct:isReferencedBy F2021L00334: ;
    rdfs:comment "Endnote 3 Legislation history - Abrievated Graph Key: I430"@en-AU ;
    skos:definition "Endnote 3 Legislation history"@en-AU ;
    skos:narrower F2021L00334:427 ;
    skos:prefLabel "Item I430"@en-AU ;
    dcat:accessURL <https://www.legislation.gov.au/F2021L00334/2023-08-04/2023-08-04/text/original/epub/OEBPS/document_1/document_1.html#_Toc143508077> ;
    dcat:landingPage "https://www.legislation.gov.au/F2021L00334/2023-08-04/2023-08-04/text/original/epub/OEBPS/document_1/document_1.html#_Toc143508077"^^xsd:anyURI ;
    dcat:theme legcons:Item .

F2021L00334:431 a legcons:Item,
        owl:Class,
        dcat:Resource ;
    rdfs:label "Item - I431 Endnote 4 Amendment history"@en-AU ;
    dct:isPartOf F2021L00334:427 ;
    dct:isReferencedBy F2021L00334: ;
    rdfs:comment "Endnote 4 Amendment history - Abrievated Graph Key: I431"@en-AU ;
    skos:definition "Endnote 4 Amendment history"@en-AU ;
    skos:narrower F2021L00334:427 ;
    skos:prefLabel "Item I431"@en-AU ;
    dcat:accessURL <https://www.legislation.gov.au/F2021L00334/2023-08-04/2023-08-04/text/original/epub/OEBPS/document_1/document_1.html#_Toc143508078> ;
    dcat:landingPage "https://www.legislation.gov.au/F2021L00334/2023-08-04/2023-08-04/text/original/epub/OEBPS/document_1/document_1.html#_Toc143508078"^^xsd:anyURI ;
    dcat:theme legcons:Item .

F2021L00334:44 a legcons:Item,
        owl:Class,
        dcat:Resource ;
    rdfs:label "Item - I44 3 4  Requirements for farms"@en-AU ;
    dct:isPartOf F2021L00334:42 ;
    dct:isReferencedBy F2021L00334: ;
    rdfs:comment "3 4  Requirements for farms - Abrievated Graph Key: I44"@en-AU ;
    skos:definition "3 4  Requirements for farms"@en-AU ;
    skos:narrower F2021L00334:42 ;
    skos:prefLabel "Item I44"@en-AU ;
    dcat:accessURL <https://www.legislation.gov.au/F2021L00334/2023-08-04/2023-08-04/text/original/epub/OEBPS/document_1/document_1.html#_Toc143507691> ;
    dcat:landingPage "https://www.legislation.gov.au/F2021L00334/2023-08-04/2023-08-04/text/original/epub/OEBPS/document_1/document_1.html#_Toc143507691"^^xsd:anyURI ;
    dcat:theme legcons:Item .

F2021L00334:45 a legcons:Item,
        owl:Class,
        dcat:Resource ;
    rdfs:label "Item - I45 3 5  Requirements for feedlots"@en-AU ;
    dct:isPartOf F2021L00334:42 ;
    dct:isReferencedBy F2021L00334: ;
    rdfs:comment "3 5  Requirements for feedlots - Abrievated Graph Key: I45"@en-AU ;
    skos:definition "3 5  Requirements for feedlots"@en-AU ;
    skos:narrower F2021L00334:42 ;
    skos:prefLabel "Item I45"@en-AU ;
    dcat:accessURL <https://www.legislation.gov.au/F2021L00334/2023-08-04/2023-08-04/text/original/epub/OEBPS/document_1/document_1.html#_Toc143507692> ;
    dcat:landingPage "https://www.legislation.gov.au/F2021L00334/2023-08-04/2023-08-04/text/original/epub/OEBPS/document_1/document_1.html#_Toc143507692"^^xsd:anyURI ;
    dcat:theme legcons:Item .

F2021L00334:46 a legcons:Item,
        owl:Class,
        dcat:Resource ;
    rdfs:label "Item - I46 3 6  Requirements for saleyards"@en-AU ;
    dct:isPartOf F2021L00334:42 ;
    dct:isReferencedBy F2021L00334: ;
    rdfs:comment "3 6  Requirements for saleyards - Abrievated Graph Key: I46"@en-AU ;
    skos:definition "3 6  Requirements for saleyards"@en-AU ;
    skos:narrower F2021L00334:42 ;
    skos:prefLabel "Item I46"@en-AU ;
    dcat:accessURL <https://www.legislation.gov.au/F2021L00334/2023-08-04/2023-08-04/text/original/epub/OEBPS/document_1/document_1.html#_Toc143507693> ;
    dcat:landingPage "https://www.legislation.gov.au/F2021L00334/2023-08-04/2023-08-04/text/original/epub/OEBPS/document_1/document_1.html#_Toc143507693"^^xsd:anyURI ;
    dcat:theme legcons:Item .

F2021L00334:48 a legcons:Item,
        owl:Class,
        dcat:Resource ;
    rdfs:label "Item - I48 3 7  Other information to be stated in notice of decision to accredit property"@en-AU ;
    dct:isPartOf F2021L00334:47 ;
    dct:isReferencedBy F2021L00334: ;
    rdfs:comment "3 7  Other information to be stated in notice of decision to accredit property - Abrievated Graph Key: I48"@en-AU ;
    skos:definition "3 7  Other information to be stated in notice of decision to accredit property"@en-AU ;
    skos:narrower F2021L00334:47 ;
    skos:prefLabel "Item I48"@en-AU ;
    dcat:accessURL <https://www.legislation.gov.au/F2021L00334/2023-08-04/2023-08-04/text/original/epub/OEBPS/document_1/document_1.html#_Toc143507695> ;
    dcat:landingPage "https://www.legislation.gov.au/F2021L00334/2023-08-04/2023-08-04/text/original/epub/OEBPS/document_1/document_1.html#_Toc143507695"^^xsd:anyURI ;
    dcat:theme legcons:Item .

F2021L00334:49 a legcons:Item,
        owl:Class,
        dcat:Resource ;
    rdfs:label "Item - I49 3 8  Period of effect of accreditation of farm"@en-AU ;
    dct:isPartOf F2021L00334:47 ;
    dct:isReferencedBy F2021L00334: ;
    rdfs:comment "3 8  Period of effect of accreditation of farm - Abrievated Graph Key: I49"@en-AU ;
    skos:definition "3 8  Period of effect of accreditation of farm"@en-AU ;
    skos:narrower F2021L00334:47 ;
    skos:prefLabel "Item I49"@en-AU ;
    dcat:accessURL <https://www.legislation.gov.au/F2021L00334/2023-08-04/2023-08-04/text/original/epub/OEBPS/document_1/document_1.html#_Toc143507696> ;
    dcat:landingPage "https://www.legislation.gov.au/F2021L00334/2023-08-04/2023-08-04/text/original/epub/OEBPS/document_1/document_1.html#_Toc143507696"^^xsd:anyURI ;
    dcat:theme legcons:Item .

F2021L00334:5 a legcons:Item,
        owl:Class,
        dcat:Resource ;
    rdfs:label "Item - I5 1 4  Simplified outline of this instrument"@en-AU ;
    dct:isPartOf F2021L00334:1 ;
    dct:isReferencedBy F2021L00334: ;
    rdfs:comment "1 4  Simplified outline of this instrument - Abrievated Graph Key: I5"@en-AU ;
    skos:definition "1 4  Simplified outline of this instrument"@en-AU ;
    skos:narrower F2021L00334:1 ;
    skos:prefLabel "Item I5"@en-AU ;
    dcat:accessURL <https://www.legislation.gov.au/F2021L00334/2023-08-04/2023-08-04/text/original/epub/OEBPS/document_1/document_1.html#_Toc143507652> ;
    dcat:landingPage "https://www.legislation.gov.au/F2021L00334/2023-08-04/2023-08-04/text/original/epub/OEBPS/document_1/document_1.html#_Toc143507652"^^xsd:anyURI ;
    dcat:theme legcons:Item .

F2021L00334:52 a legcons:Item,
        owl:Class,
        dcat:Resource ;
    rdfs:label "Item - I52 3 9  Purpose of this Division"@en-AU ;
    dct:isPartOf F2021L00334:51 ;
    dct:isReferencedBy F2021L00334: ;
    rdfs:comment "3 9  Purpose of this Division - Abrievated Graph Key: I52"@en-AU ;
    skos:definition "3 9  Purpose of this Division"@en-AU ;
    skos:narrower F2021L00334:51 ;
    skos:prefLabel "Item I52"@en-AU ;
    dcat:accessURL <https://www.legislation.gov.au/F2021L00334/2023-08-04/2023-08-04/text/original/epub/OEBPS/document_1/document_1.html#_Toc143507699> ;
    dcat:landingPage "https://www.legislation.gov.au/F2021L00334/2023-08-04/2023-08-04/text/original/epub/OEBPS/document_1/document_1.html#_Toc143507699"^^xsd:anyURI ;
    dcat:theme legcons:Item .

F2021L00334:53 a legcons:Item,
        owl:Class,
        dcat:Resource ;
    rdfs:label "Item - I53 3 10  Requirements for accreditation continue to be met"@en-AU ;
    dct:isPartOf F2021L00334:51 ;
    dct:isReferencedBy F2021L00334: ;
    rdfs:comment "3 10  Requirements for accreditation continue to be met - Abrievated Graph Key: I53"@en-AU ;
    skos:definition "3 10  Requirements for accreditation continue to be met"@en-AU ;
    skos:narrower F2021L00334:51 ;
    skos:prefLabel "Item I53"@en-AU ;
    dcat:accessURL <https://www.legislation.gov.au/F2021L00334/2023-08-04/2023-08-04/text/original/epub/OEBPS/document_1/document_1.html#_Toc143507700> ;
    dcat:landingPage "https://www.legislation.gov.au/F2021L00334/2023-08-04/2023-08-04/text/original/epub/OEBPS/document_1/document_1.html#_Toc143507700"^^xsd:anyURI ;
    dcat:theme legcons:Item .

F2021L00334:54 a legcons:Item,
        owl:Class,
        dcat:Resource ;
    rdfs:label "Item - I54 3 11  Identification and traceability"@en-AU ;
    dct:isPartOf F2021L00334:51 ;
    dct:isReferencedBy F2021L00334: ;
    rdfs:comment "3 11  Identification and traceability - Abrievated Graph Key: I54"@en-AU ;
    skos:definition "3 11  Identification and traceability"@en-AU ;
    skos:narrower F2021L00334:51 ;
    skos:prefLabel "Item I54"@en-AU ;
    dcat:accessURL <https://www.legislation.gov.au/F2021L00334/2023-08-04/2023-08-04/text/original/epub/OEBPS/document_1/document_1.html#_Toc143507701> ;
    dcat:landingPage "https://www.legislation.gov.au/F2021L00334/2023-08-04/2023-08-04/text/original/epub/OEBPS/document_1/document_1.html#_Toc143507701"^^xsd:anyURI ;
    dcat:theme legcons:Item .

F2021L00334:55 a legcons:Item,
        owl:Class,
        dcat:Resource ;
    rdfs:label "Item - I55 3 12  Bovine animals must not be treated with an HGP"@en-AU ;
    dct:isPartOf F2021L00334:51 ;
    dct:isReferencedBy F2021L00334: ;
    rdfs:comment "3 12  Bovine animals must not be treated with an HGP - Abrievated Graph Key: I55"@en-AU ;
    skos:definition "3 12  Bovine animals must not be treated with an HGP"@en-AU ;
    skos:narrower F2021L00334:51 ;
    skos:prefLabel "Item I55"@en-AU ;
    dcat:accessURL <https://www.legislation.gov.au/F2021L00334/2023-08-04/2023-08-04/text/original/epub/OEBPS/document_1/document_1.html#_Toc143507702> ;
    dcat:landingPage "https://www.legislation.gov.au/F2021L00334/2023-08-04/2023-08-04/text/original/epub/OEBPS/document_1/document_1.html#_Toc143507702"^^xsd:anyURI ;
    dcat:theme legcons:Item .

F2021L00334:56 a legcons:Item,
        owl:Class,
        dcat:Resource ;
    rdfs:label "Item - I56 3 13  Integrity"@en-AU ;
    dct:isPartOf F2021L00334:51 ;
    dct:isReferencedBy F2021L00334: ;
    rdfs:comment "3 13  Integrity - Abrievated Graph Key: I56"@en-AU ;
    skos:definition "3 13  Integrity"@en-AU ;
    skos:narrower F2021L00334:51 ;
    skos:prefLabel "Item I56"@en-AU ;
    dcat:accessURL <https://www.legislation.gov.au/F2021L00334/2023-08-04/2023-08-04/text/original/epub/OEBPS/document_1/document_1.html#_Toc143507703> ;
    dcat:landingPage "https://www.legislation.gov.au/F2021L00334/2023-08-04/2023-08-04/text/original/epub/OEBPS/document_1/document_1.html#_Toc143507703"^^xsd:anyURI ;
    dcat:theme legcons:Item .

F2021L00334:57 a legcons:Item,
        owl:Class,
        dcat:Resource ;
    rdfs:label "Item - I57 3 14  Records"@en-AU ;
    dct:isPartOf F2021L00334:51 ;
    dct:isReferencedBy F2021L00334: ;
    rdfs:comment "3 14  Records - Abrievated Graph Key: I57"@en-AU ;
    skos:definition "3 14  Records"@en-AU ;
    skos:narrower F2021L00334:51 ;
    skos:prefLabel "Item I57"@en-AU ;
    dcat:accessURL <https://www.legislation.gov.au/F2021L00334/2023-08-04/2023-08-04/text/original/epub/OEBPS/document_1/document_1.html#_Toc143507704> ;
    dcat:landingPage "https://www.legislation.gov.au/F2021L00334/2023-08-04/2023-08-04/text/original/epub/OEBPS/document_1/document_1.html#_Toc143507704"^^xsd:anyURI ;
    dcat:theme legcons:Item .

F2021L00334:59 a legcons:Item,
        owl:Class,
        dcat:Resource ;
    rdfs:label "Item - I59 3 15  Purpose of this Division"@en-AU ;
    dct:isPartOf F2021L00334:58 ;
    dct:isReferencedBy F2021L00334: ;
    rdfs:comment "3 15  Purpose of this Division - Abrievated Graph Key: I59"@en-AU ;
    skos:definition "3 15  Purpose of this Division"@en-AU ;
    skos:narrower F2021L00334:58 ;
    skos:prefLabel "Item I59"@en-AU ;
    dcat:accessURL <https://www.legislation.gov.au/F2021L00334/2023-08-04/2023-08-04/text/original/epub/OEBPS/document_1/document_1.html#_Toc143507706> ;
    dcat:landingPage "https://www.legislation.gov.au/F2021L00334/2023-08-04/2023-08-04/text/original/epub/OEBPS/document_1/document_1.html#_Toc143507706"^^xsd:anyURI ;
    dcat:theme legcons:Item .

F2021L00334:6 a legcons:Part,
        owl:Class,
        dcat:Resource ;
    rdfs:label "Part - P6 Part 2 Interpretation"@en-AU ;
    dct:isPartOf F2021L00334:1 ;
    dct:isReferencedBy F2021L00334: ;
    rdfs:comment "Part 2 Interpretation - Abrievated Graph Key: P6"@en-AU ;
    skos:definition "Part 2 Interpretation"@en-AU ;
    skos:narrower F2021L00334:1 ;
    skos:prefLabel "Part P6"@en-AU ;
    dcat:accessURL <https://www.legislation.gov.au/F2021L00334/2023-08-04/2023-08-04/text/original/epub/OEBPS/document_1/document_1.html#_Toc143507653> ;
    dcat:landingPage "https://www.legislation.gov.au/F2021L00334/2023-08-04/2023-08-04/text/original/epub/OEBPS/document_1/document_1.html#_Toc143507653"^^xsd:anyURI ;
    dcat:theme legcons:Part .

F2021L00334:60 a legcons:Item,
        owl:Class,
        dcat:Resource ;
    rdfs:label "Item - I60 3 16  Requirements for accreditation continue to be met"@en-AU ;
    dct:isPartOf F2021L00334:58 ;
    dct:isReferencedBy F2021L00334: ;
    rdfs:comment "3 16  Requirements for accreditation continue to be met - Abrievated Graph Key: I60"@en-AU ;
    skos:definition "3 16  Requirements for accreditation continue to be met"@en-AU ;
    skos:narrower F2021L00334:58 ;
    skos:prefLabel "Item I60"@en-AU ;
    dcat:accessURL <https://www.legislation.gov.au/F2021L00334/2023-08-04/2023-08-04/text/original/epub/OEBPS/document_1/document_1.html#_Toc143507707> ;
    dcat:landingPage "https://www.legislation.gov.au/F2021L00334/2023-08-04/2023-08-04/text/original/epub/OEBPS/document_1/document_1.html#_Toc143507707"^^xsd:anyURI ;
    dcat:theme legcons:Item .

F2021L00334:61 a legcons:Item,
        owl:Class,
        dcat:Resource ;
    rdfs:label "Item - I61 3 17  Identification traceability and integrity"@en-AU ;
    dct:isPartOf F2021L00334:58 ;
    dct:isReferencedBy F2021L00334: ;
    rdfs:comment "3 17  Identification traceability and integrity - Abrievated Graph Key: I61"@en-AU ;
    skos:definition "3 17  Identification traceability and integrity"@en-AU ;
    skos:narrower F2021L00334:58 ;
    skos:prefLabel "Item I61"@en-AU ;
    dcat:accessURL <https://www.legislation.gov.au/F2021L00334/2023-08-04/2023-08-04/text/original/epub/OEBPS/document_1/document_1.html#_Toc143507708> ;
    dcat:landingPage "https://www.legislation.gov.au/F2021L00334/2023-08-04/2023-08-04/text/original/epub/OEBPS/document_1/document_1.html#_Toc143507708"^^xsd:anyURI ;
    dcat:theme legcons:Item .

F2021L00334:62 a legcons:Item,
        owl:Class,
        dcat:Resource ;
    rdfs:label "Item - I62 3 18  Feedlot management system must be implemented"@en-AU ;
    dct:isPartOf F2021L00334:58 ;
    dct:isReferencedBy F2021L00334: ;
    rdfs:comment "3 18  Feedlot management system must be implemented - Abrievated Graph Key: I62"@en-AU ;
    skos:definition "3 18  Feedlot management system must be implemented"@en-AU ;
    skos:narrower F2021L00334:58 ;
    skos:prefLabel "Item I62"@en-AU ;
    dcat:accessURL <https://www.legislation.gov.au/F2021L00334/2023-08-04/2023-08-04/text/original/epub/OEBPS/document_1/document_1.html#_Toc143507709> ;
    dcat:landingPage "https://www.legislation.gov.au/F2021L00334/2023-08-04/2023-08-04/text/original/epub/OEBPS/document_1/document_1.html#_Toc143507709"^^xsd:anyURI ;
    dcat:theme legcons:Item .

F2021L00334:63 a legcons:Item,
        owl:Class,
        dcat:Resource ;
    rdfs:label "Item - I63 3 19  Records"@en-AU ;
    dct:isPartOf F2021L00334:58 ;
    dct:isReferencedBy F2021L00334: ;
    rdfs:comment "3 19  Records - Abrievated Graph Key: I63"@en-AU ;
    skos:definition "3 19  Records"@en-AU ;
    skos:narrower F2021L00334:58 ;
    skos:prefLabel "Item I63"@en-AU ;
    dcat:accessURL <https://www.legislation.gov.au/F2021L00334/2023-08-04/2023-08-04/text/original/epub/OEBPS/document_1/document_1.html#_Toc143507710> ;
    dcat:landingPage "https://www.legislation.gov.au/F2021L00334/2023-08-04/2023-08-04/text/original/epub/OEBPS/document_1/document_1.html#_Toc143507710"^^xsd:anyURI ;
    dcat:theme legcons:Item .

F2021L00334:65 a legcons:Item,
        owl:Class,
        dcat:Resource ;
    rdfs:label "Item - I65 3 20  Purpose of this Division"@en-AU ;
    dct:isPartOf F2021L00334:64 ;
    dct:isReferencedBy F2021L00334: ;
    rdfs:comment "3 20  Purpose of this Division - Abrievated Graph Key: I65"@en-AU ;
    skos:definition "3 20  Purpose of this Division"@en-AU ;
    skos:narrower F2021L00334:64 ;
    skos:prefLabel "Item I65"@en-AU ;
    dcat:accessURL <https://www.legislation.gov.au/F2021L00334/2023-08-04/2023-08-04/text/original/epub/OEBPS/document_1/document_1.html#_Toc143507712> ;
    dcat:landingPage "https://www.legislation.gov.au/F2021L00334/2023-08-04/2023-08-04/text/original/epub/OEBPS/document_1/document_1.html#_Toc143507712"^^xsd:anyURI ;
    dcat:theme legcons:Item .

F2021L00334:66 a legcons:Item,
        owl:Class,
        dcat:Resource ;
    rdfs:label "Item - I66 3 21  Requirements for accreditation continue to be met"@en-AU ;
    dct:isPartOf F2021L00334:64 ;
    dct:isReferencedBy F2021L00334: ;
    rdfs:comment "3 21  Requirements for accreditation continue to be met - Abrievated Graph Key: I66"@en-AU ;
    skos:definition "3 21  Requirements for accreditation continue to be met"@en-AU ;
    skos:narrower F2021L00334:64 ;
    skos:prefLabel "Item I66"@en-AU ;
    dcat:accessURL <https://www.legislation.gov.au/F2021L00334/2023-08-04/2023-08-04/text/original/epub/OEBPS/document_1/document_1.html#_Toc143507713> ;
    dcat:landingPage "https://www.legislation.gov.au/F2021L00334/2023-08-04/2023-08-04/text/original/epub/OEBPS/document_1/document_1.html#_Toc143507713"^^xsd:anyURI ;
    dcat:theme legcons:Item .

F2021L00334:67 a legcons:Item,
        owl:Class,
        dcat:Resource ;
    rdfs:label "Item - I67 3 22  Identification and traceability"@en-AU ;
    dct:isPartOf F2021L00334:64 ;
    dct:isReferencedBy F2021L00334: ;
    rdfs:comment "3 22  Identification and traceability - Abrievated Graph Key: I67"@en-AU ;
    skos:definition "3 22  Identification and traceability"@en-AU ;
    skos:narrower F2021L00334:64 ;
    skos:prefLabel "Item I67"@en-AU ;
    dcat:accessURL <https://www.legislation.gov.au/F2021L00334/2023-08-04/2023-08-04/text/original/epub/OEBPS/document_1/document_1.html#_Toc143507714> ;
    dcat:landingPage "https://www.legislation.gov.au/F2021L00334/2023-08-04/2023-08-04/text/original/epub/OEBPS/document_1/document_1.html#_Toc143507714"^^xsd:anyURI ;
    dcat:theme legcons:Item .

F2021L00334:68 a legcons:Item,
        owl:Class,
        dcat:Resource ;
    rdfs:label "Item - I68 3 23  Bovine animals must not be treated with an HGP"@en-AU ;
    dct:isPartOf F2021L00334:64 ;
    dct:isReferencedBy F2021L00334: ;
    rdfs:comment "3 23  Bovine animals must not be treated with an HGP - Abrievated Graph Key: I68"@en-AU ;
    skos:definition "3 23  Bovine animals must not be treated with an HGP"@en-AU ;
    skos:narrower F2021L00334:64 ;
    skos:prefLabel "Item I68"@en-AU ;
    dcat:accessURL <https://www.legislation.gov.au/F2021L00334/2023-08-04/2023-08-04/text/original/epub/OEBPS/document_1/document_1.html#_Toc143507715> ;
    dcat:landingPage "https://www.legislation.gov.au/F2021L00334/2023-08-04/2023-08-04/text/original/epub/OEBPS/document_1/document_1.html#_Toc143507715"^^xsd:anyURI ;
    dcat:theme legcons:Item .

F2021L00334:69 a legcons:Item,
        owl:Class,
        dcat:Resource ;
    rdfs:label "Item - I69 3 24  Saleyard management system must be implemented"@en-AU ;
    dct:isPartOf F2021L00334:64 ;
    dct:isReferencedBy F2021L00334: ;
    rdfs:comment "3 24  Saleyard management system must be implemented - Abrievated Graph Key: I69"@en-AU ;
    skos:definition "3 24  Saleyard management system must be implemented"@en-AU ;
    skos:narrower F2021L00334:64 ;
    skos:prefLabel "Item I69"@en-AU ;
    dcat:accessURL <https://www.legislation.gov.au/F2021L00334/2023-08-04/2023-08-04/text/original/epub/OEBPS/document_1/document_1.html#_Toc143507716> ;
    dcat:landingPage "https://www.legislation.gov.au/F2021L00334/2023-08-04/2023-08-04/text/original/epub/OEBPS/document_1/document_1.html#_Toc143507716"^^xsd:anyURI ;
    dcat:theme legcons:Item .

F2021L00334:7 a legcons:Division,
        owl:Class,
        dcat:Resource ;
    rdfs:label "Division - D7 Division 1 Definitions"@en-AU ;
    dct:isPartOf F2021L00334:1 ;
    dct:isReferencedBy F2021L00334: ;
    rdfs:comment "Division 1 Definitions - Abrievated Graph Key: D7"@en-AU ;
    skos:definition "Division 1 Definitions"@en-AU ;
    skos:narrower F2021L00334:1 ;
    skos:prefLabel "Division D7"@en-AU ;
    dcat:accessURL <https://www.legislation.gov.au/F2021L00334/2023-08-04/2023-08-04/text/original/epub/OEBPS/document_1/document_1.html#_Toc143507654> ;
    dcat:landingPage "https://www.legislation.gov.au/F2021L00334/2023-08-04/2023-08-04/text/original/epub/OEBPS/document_1/document_1.html#_Toc143507654"^^xsd:anyURI ;
    dcat:theme legcons:Division .

F2021L00334:70 a legcons:Item,
        owl:Class,
        dcat:Resource ;
    rdfs:label "Item - I70 3 25  Records"@en-AU ;
    dct:isPartOf F2021L00334:64 ;
    dct:isReferencedBy F2021L00334: ;
    rdfs:comment "3 25  Records - Abrievated Graph Key: I70"@en-AU ;
    skos:definition "3 25  Records"@en-AU ;
    skos:narrower F2021L00334:64 ;
    skos:prefLabel "Item I70"@en-AU ;
    dcat:accessURL <https://www.legislation.gov.au/F2021L00334/2023-08-04/2023-08-04/text/original/epub/OEBPS/document_1/document_1.html#_Toc143507717> ;
    dcat:landingPage "https://www.legislation.gov.au/F2021L00334/2023-08-04/2023-08-04/text/original/epub/OEBPS/document_1/document_1.html#_Toc143507717"^^xsd:anyURI ;
    dcat:theme legcons:Item .

F2021L00334:72 a legcons:Item,
        owl:Class,
        dcat:Resource ;
    rdfs:label "Item - I72 3 26  Period within which application to renew accreditation must be made"@en-AU ;
    dct:isPartOf F2021L00334:71 ;
    dct:isReferencedBy F2021L00334: ;
    rdfs:comment "3 26  Period within which application to renew accreditation must be made - Abrievated Graph Key: I72"@en-AU ;
    skos:definition "3 26  Period within which application to renew accreditation must be made"@en-AU ;
    skos:narrower F2021L00334:71 ;
    skos:prefLabel "Item I72"@en-AU ;
    dcat:accessURL <https://www.legislation.gov.au/F2021L00334/2023-08-04/2023-08-04/text/original/epub/OEBPS/document_1/document_1.html#_Toc143507719> ;
    dcat:landingPage "https://www.legislation.gov.au/F2021L00334/2023-08-04/2023-08-04/text/original/epub/OEBPS/document_1/document_1.html#_Toc143507719"^^xsd:anyURI ;
    dcat:theme legcons:Item .

F2021L00334:73 a legcons:Item,
        owl:Class,
        dcat:Resource ;
    rdfs:label "Item - I73 3 27  Conditions of renewed accreditation"@en-AU ;
    dct:isPartOf F2021L00334:71 ;
    dct:isReferencedBy F2021L00334: ;
    rdfs:comment "3 27  Conditions of renewed accreditation - Abrievated Graph Key: I73"@en-AU ;
    skos:definition "3 27  Conditions of renewed accreditation"@en-AU ;
    skos:narrower F2021L00334:71 ;
    skos:prefLabel "Item I73"@en-AU ;
    dcat:accessURL <https://www.legislation.gov.au/F2021L00334/2023-08-04/2023-08-04/text/original/epub/OEBPS/document_1/document_1.html#_Toc143507720> ;
    dcat:landingPage "https://www.legislation.gov.au/F2021L00334/2023-08-04/2023-08-04/text/original/epub/OEBPS/document_1/document_1.html#_Toc143507720"^^xsd:anyURI ;
    dcat:theme legcons:Item .

F2021L00334:75 a legcons:Item,
        owl:Class,
        dcat:Resource ;
    rdfs:label "Item - I75 3 28  Alteration of boundaries of property other than because of increase in area"@en-AU ;
    dct:isPartOf F2021L00334:74 ;
    dct:isReferencedBy F2021L00334: ;
    rdfs:comment "3 28  Alteration of boundaries of property other than because of increase in area - Abrievated Graph Key: I75"@en-AU ;
    skos:definition "3 28  Alteration of boundaries of property other than because of increase in area"@en-AU ;
    skos:narrower F2021L00334:74 ;
    skos:prefLabel "Item I75"@en-AU ;
    dcat:accessURL <https://www.legislation.gov.au/F2021L00334/2023-08-04/2023-08-04/text/original/epub/OEBPS/document_1/document_1.html#_Toc143507722> ;
    dcat:landingPage "https://www.legislation.gov.au/F2021L00334/2023-08-04/2023-08-04/text/original/epub/OEBPS/document_1/document_1.html#_Toc143507722"^^xsd:anyURI ;
    dcat:theme legcons:Item .

F2021L00334:76 a legcons:Item,
        owl:Class,
        dcat:Resource ;
    rdfs:label "Item - I76 3 29  Carrying out export operations on additional part of property or on another property"@en-AU ;
    dct:isPartOf F2021L00334:74 ;
    dct:isReferencedBy F2021L00334: ;
    rdfs:comment "3 29  Carrying out export operations on additional part of property or on another property - Abrievated Graph Key: I76"@en-AU ;
    skos:definition "3 29  Carrying out export operations on additional part of property or on another property"@en-AU ;
    skos:narrower F2021L00334:74 ;
    skos:prefLabel "Item I76"@en-AU ;
    dcat:accessURL <https://www.legislation.gov.au/F2021L00334/2023-08-04/2023-08-04/text/original/epub/OEBPS/document_1/document_1.html#_Toc143507723> ;
    dcat:landingPage "https://www.legislation.gov.au/F2021L00334/2023-08-04/2023-08-04/text/original/epub/OEBPS/document_1/document_1.html#_Toc143507723"^^xsd:anyURI ;
    dcat:theme legcons:Item .

F2021L00334:78 a legcons:Item,
        owl:Class,
        dcat:Resource ;
    rdfs:label "Item - I78 3 30  Other grounds for revocation"@en-AU ;
    dct:isPartOf F2021L00334:77 ;
    dct:isReferencedBy F2021L00334: ;
    rdfs:comment "3 30  Other grounds for revocation - Abrievated Graph Key: I78"@en-AU ;
    skos:definition "3 30  Other grounds for revocation"@en-AU ;
    skos:narrower F2021L00334:77 ;
    skos:prefLabel "Item I78"@en-AU ;
    dcat:accessURL <https://www.legislation.gov.au/F2021L00334/2023-08-04/2023-08-04/text/original/epub/OEBPS/document_1/document_1.html#_Toc143507725> ;
    dcat:landingPage "https://www.legislation.gov.au/F2021L00334/2023-08-04/2023-08-04/text/original/epub/OEBPS/document_1/document_1.html#_Toc143507725"^^xsd:anyURI ;
    dcat:theme legcons:Item .

F2021L00334:8 a legcons:Item,
        owl:Class,
        dcat:Resource ;
    rdfs:label "Item - I8 1 5  Definitions"@en-AU ;
    dct:isPartOf F2021L00334:1 ;
    dct:isReferencedBy F2021L00334: ;
    rdfs:comment "1 5  Definitions - Abrievated Graph Key: I8"@en-AU ;
    skos:definition "1 5  Definitions"@en-AU ;
    skos:narrower F2021L00334:1 ;
    skos:prefLabel "Item I8"@en-AU ;
    dcat:accessURL <https://www.legislation.gov.au/F2021L00334/2023-08-04/2023-08-04/text/original/epub/OEBPS/document_1/document_1.html#_Toc143507655> ;
    dcat:landingPage "https://www.legislation.gov.au/F2021L00334/2023-08-04/2023-08-04/text/original/epub/OEBPS/document_1/document_1.html#_Toc143507655"^^xsd:anyURI ;
    dcat:theme legcons:Item .

F2021L00334:80 a legcons:Item,
        owl:Class,
        dcat:Resource ;
    rdfs:label "Item - I80 3 31  Circumstances of which Secretary must be notified"@en-AU ;
    dct:isPartOf F2021L00334:79 ;
    dct:isReferencedBy F2021L00334: ;
    rdfs:comment "3 31  Circumstances of which Secretary must be notified - Abrievated Graph Key: I80"@en-AU ;
    skos:definition "3 31  Circumstances of which Secretary must be notified"@en-AU ;
    skos:narrower F2021L00334:79 ;
    skos:prefLabel "Item I80"@en-AU ;
    dcat:accessURL <https://www.legislation.gov.au/F2021L00334/2023-08-04/2023-08-04/text/original/epub/OEBPS/document_1/document_1.html#_Toc143507727> ;
    dcat:landingPage "https://www.legislation.gov.au/F2021L00334/2023-08-04/2023-08-04/text/original/epub/OEBPS/document_1/document_1.html#_Toc143507727"^^xsd:anyURI ;
    dcat:theme legcons:Item .

F2021L00334:81 a legcons:Item,
        owl:Class,
        dcat:Resource ;
    rdfs:label "Item - I81 3 32  Accredited properties that no longer have a manager or in relation to which manager has changed"@en-AU ;
    dct:isPartOf F2021L00334:79 ;
    dct:isReferencedBy F2021L00334: ;
    rdfs:comment "3 32  Accredited properties that no longer have a manager or in relation to which manager has changed - Abrievated Graph Key: I81"@en-AU ;
    skos:definition "3 32  Accredited properties that no longer have a manager or in relation to which manager has changed"@en-AU ;
    skos:narrower F2021L00334:79 ;
    skos:prefLabel "Item I81"@en-AU ;
    dcat:accessURL <https://www.legislation.gov.au/F2021L00334/2023-08-04/2023-08-04/text/original/epub/OEBPS/document_1/document_1.html#_Toc143507728> ;
    dcat:landingPage "https://www.legislation.gov.au/F2021L00334/2023-08-04/2023-08-04/text/original/epub/OEBPS/document_1/document_1.html#_Toc143507728"^^xsd:anyURI ;
    dcat:theme legcons:Item .

F2021L00334:83 a legcons:Item,
        owl:Class,
        dcat:Resource ;
    rdfs:label "Item - I83 3 33  Application of this Part"@en-AU ;
    dct:isPartOf F2021L00334:82 ;
    dct:isReferencedBy F2021L00334: ;
    rdfs:comment "3 33  Application of this Part - Abrievated Graph Key: I83"@en-AU ;
    skos:definition "3 33  Application of this Part"@en-AU ;
    skos:narrower F2021L00334:82 ;
    skos:prefLabel "Item I83"@en-AU ;
    dcat:accessURL <https://www.legislation.gov.au/F2021L00334/2023-08-04/2023-08-04/text/original/epub/OEBPS/document_1/document_1.html#_Toc143507730> ;
    dcat:landingPage "https://www.legislation.gov.au/F2021L00334/2023-08-04/2023-08-04/text/original/epub/OEBPS/document_1/document_1.html#_Toc143507730"^^xsd:anyURI ;
    dcat:theme legcons:Item .

F2021L00334:84 a legcons:Item,
        owl:Class,
        dcat:Resource ;
    rdfs:label "Item - I84 3 34  Documents to accompany application"@en-AU ;
    dct:isPartOf F2021L00334:82 ;
    dct:isReferencedBy F2021L00334: ;
    rdfs:comment "3 34  Documents to accompany application - Abrievated Graph Key: I84"@en-AU ;
    skos:definition "3 34  Documents to accompany application"@en-AU ;
    skos:narrower F2021L00334:82 ;
    skos:prefLabel "Item I84"@en-AU ;
    dcat:accessURL <https://www.legislation.gov.au/F2021L00334/2023-08-04/2023-08-04/text/original/epub/OEBPS/document_1/document_1.html#_Toc143507731> ;
    dcat:landingPage "https://www.legislation.gov.au/F2021L00334/2023-08-04/2023-08-04/text/original/epub/OEBPS/document_1/document_1.html#_Toc143507731"^^xsd:anyURI ;
    dcat:theme legcons:Item .

F2021L00334:85 a legcons:Item,
        owl:Class,
        dcat:Resource ;
    rdfs:label "Item - I85 3 35  Initial consideration period"@en-AU ;
    dct:isPartOf F2021L00334:82 ;
    dct:isReferencedBy F2021L00334: ;
    rdfs:comment "3 35  Initial consideration period - Abrievated Graph Key: I85"@en-AU ;
    skos:definition "3 35  Initial consideration period"@en-AU ;
    skos:narrower F2021L00334:82 ;
    skos:prefLabel "Item I85"@en-AU ;
    dcat:accessURL <https://www.legislation.gov.au/F2021L00334/2023-08-04/2023-08-04/text/original/epub/OEBPS/document_1/document_1.html#_Toc143507732> ;
    dcat:landingPage "https://www.legislation.gov.au/F2021L00334/2023-08-04/2023-08-04/text/original/epub/OEBPS/document_1/document_1.html#_Toc143507732"^^xsd:anyURI ;
    dcat:theme legcons:Item .

F2021L00334:86 a legcons:Item,
        owl:Class,
        dcat:Resource ;
    rdfs:label "Item - I86 3 36  Period within which request relating to application must be complied with"@en-AU ;
    dct:isPartOf F2021L00334:82 ;
    dct:isReferencedBy F2021L00334: ;
    rdfs:comment "3 36  Period within which request relating to application must be complied with - Abrievated Graph Key: I86"@en-AU ;
    skos:definition "3 36  Period within which request relating to application must be complied with"@en-AU ;
    skos:narrower F2021L00334:82 ;
    skos:prefLabel "Item I86"@en-AU ;
    dcat:accessURL <https://www.legislation.gov.au/F2021L00334/2023-08-04/2023-08-04/text/original/epub/OEBPS/document_1/document_1.html#_Toc143507733> ;
    dcat:landingPage "https://www.legislation.gov.au/F2021L00334/2023-08-04/2023-08-04/text/original/epub/OEBPS/document_1/document_1.html#_Toc143507733"^^xsd:anyURI ;
    dcat:theme legcons:Item .

F2021L00334:89 a legcons:Item,
        owl:Class,
        dcat:Resource ;
    rdfs:label "Item - I89 4 1  Purpose of this Part"@en-AU ;
    dct:isPartOf F2021L00334:88 ;
    dct:isReferencedBy F2021L00334: ;
    rdfs:comment "4 1  Purpose of this Part - Abrievated Graph Key: I89"@en-AU ;
    skos:definition "4 1  Purpose of this Part"@en-AU ;
    skos:narrower F2021L00334:88 ;
    skos:prefLabel "Item I89"@en-AU ;
    dcat:accessURL <https://www.legislation.gov.au/F2021L00334/2023-08-04/2023-08-04/text/original/epub/OEBPS/document_1/document_1.html#_Toc143507736> ;
    dcat:landingPage "https://www.legislation.gov.au/F2021L00334/2023-08-04/2023-08-04/text/original/epub/OEBPS/document_1/document_1.html#_Toc143507736"^^xsd:anyURI ;
    dcat:theme legcons:Item .

F2021L00334:9 a legcons:Item,
        owl:Class,
        dcat:Resource ;
    rdfs:label "Item - I9 1 6  Meaning of loaded for export"@en-AU ;
    dct:isPartOf F2021L00334:1 ;
    dct:isReferencedBy F2021L00334: ;
    rdfs:comment "1 6  Meaning of loaded for export - Abrievated Graph Key: I9"@en-AU ;
    skos:definition "1 6  Meaning of loaded for export"@en-AU ;
    skos:narrower F2021L00334:1 ;
    skos:prefLabel "Item I9"@en-AU ;
    dcat:accessURL <https://www.legislation.gov.au/F2021L00334/2023-08-04/2023-08-04/text/original/epub/OEBPS/document_1/document_1.html#_Toc143507656> ;
    dcat:landingPage "https://www.legislation.gov.au/F2021L00334/2023-08-04/2023-08-04/text/original/epub/OEBPS/document_1/document_1.html#_Toc143507656"^^xsd:anyURI ;
    dcat:theme legcons:Item .

F2021L00334:90 a legcons:Item,
        owl:Class,
        dcat:Resource ;
    rdfs:label "Item - I90 4 2  Operations must be carried out in a way that will ensure requirements of the Act are complied with"@en-AU ;
    dct:isPartOf F2021L00334:88 ;
    dct:isReferencedBy F2021L00334: ;
    rdfs:comment "4 2  Operations must be carried out in a way that will ensure requirements of the Act are complied with - Abrievated Graph Key: I90"@en-AU ;
    skos:definition "4 2  Operations must be carried out in a way that will ensure requirements of the Act are complied with"@en-AU ;
    skos:narrower F2021L00334:88 ;
    skos:prefLabel "Item I90"@en-AU ;
    dcat:accessURL <https://www.legislation.gov.au/F2021L00334/2023-08-04/2023-08-04/text/original/epub/OEBPS/document_1/document_1.html#_Toc143507737> ;
    dcat:landingPage "https://www.legislation.gov.au/F2021L00334/2023-08-04/2023-08-04/text/original/epub/OEBPS/document_1/document_1.html#_Toc143507737"^^xsd:anyURI ;
    dcat:theme legcons:Item .

F2021L00334:91 a legcons:Item,
        owl:Class,
        dcat:Resource ;
    rdfs:label "Item - I91 4 3  Requirements of Australian Meat Standard must be met"@en-AU ;
    dct:isPartOf F2021L00334:88 ;
    dct:isReferencedBy F2021L00334: ;
    rdfs:comment "4 3  Requirements of Australian Meat Standard must be met - Abrievated Graph Key: I91"@en-AU ;
    skos:definition "4 3  Requirements of Australian Meat Standard must be met"@en-AU ;
    skos:narrower F2021L00334:88 ;
    skos:prefLabel "Item I91"@en-AU ;
    dcat:accessURL <https://www.legislation.gov.au/F2021L00334/2023-08-04/2023-08-04/text/original/epub/OEBPS/document_1/document_1.html#_Toc143507738> ;
    dcat:landingPage "https://www.legislation.gov.au/F2021L00334/2023-08-04/2023-08-04/text/original/epub/OEBPS/document_1/document_1.html#_Toc143507738"^^xsd:anyURI ;
    dcat:theme legcons:Item .

F2021L00334:92 a legcons:Item,
        owl:Class,
        dcat:Resource ;
    rdfs:label "Item - I92 4 4  Equipment facilities and essential services"@en-AU ;
    dct:isPartOf F2021L00334:88 ;
    dct:isReferencedBy F2021L00334: ;
    rdfs:comment "4 4  Equipment facilities and essential services - Abrievated Graph Key: I92"@en-AU ;
    skos:definition "4 4  Equipment facilities and essential services"@en-AU ;
    skos:narrower F2021L00334:88 ;
    skos:prefLabel "Item I92"@en-AU ;
    dcat:accessURL <https://www.legislation.gov.au/F2021L00334/2023-08-04/2023-08-04/text/original/epub/OEBPS/document_1/document_1.html#_Toc143507739> ;
    dcat:landingPage "https://www.legislation.gov.au/F2021L00334/2023-08-04/2023-08-04/text/original/epub/OEBPS/document_1/document_1.html#_Toc143507739"^^xsd:anyURI ;
    dcat:theme legcons:Item .

F2021L00334:93 a legcons:Item,
        owl:Class,
        dcat:Resource ;
    rdfs:label "Item - I93 4 5  Areas where post mortem inspections are carried out"@en-AU ;
    dct:isPartOf F2021L00334:88 ;
    dct:isReferencedBy F2021L00334: ;
    rdfs:comment "4 5  Areas where post mortem inspections are carried out - Abrievated Graph Key: I93"@en-AU ;
    skos:definition "4 5  Areas where post mortem inspections are carried out"@en-AU ;
    skos:narrower F2021L00334:88 ;
    skos:prefLabel "Item I93"@en-AU ;
    dcat:accessURL <https://www.legislation.gov.au/F2021L00334/2023-08-04/2023-08-04/text/original/epub/OEBPS/document_1/document_1.html#_Toc143507740> ;
    dcat:landingPage "https://www.legislation.gov.au/F2021L00334/2023-08-04/2023-08-04/text/original/epub/OEBPS/document_1/document_1.html#_Toc143507740"^^xsd:anyURI ;
    dcat:theme legcons:Item .

F2021L00334:94 a legcons:Item,
        owl:Class,
        dcat:Resource ;
    rdfs:label "Item - I94 4 6  Meat examination facility"@en-AU ;
    dct:isPartOf F2021L00334:88 ;
    dct:isReferencedBy F2021L00334: ;
    rdfs:comment "4 6  Meat examination facility - Abrievated Graph Key: I94"@en-AU ;
    skos:definition "4 6  Meat examination facility"@en-AU ;
    skos:narrower F2021L00334:88 ;
    skos:prefLabel "Item I94"@en-AU ;
    dcat:accessURL <https://www.legislation.gov.au/F2021L00334/2023-08-04/2023-08-04/text/original/epub/OEBPS/document_1/document_1.html#_Toc143507741> ;
    dcat:landingPage "https://www.legislation.gov.au/F2021L00334/2023-08-04/2023-08-04/text/original/epub/OEBPS/document_1/document_1.html#_Toc143507741"^^xsd:anyURI ;
    dcat:theme legcons:Item .

F2021L00334:95 a legcons:Item,
        owl:Class,
        dcat:Resource ;
    rdfs:label "Item - I95 4 7  Slaughter establishments must have laboratory facility"@en-AU ;
    dct:isPartOf F2021L00334:88 ;
    dct:isReferencedBy F2021L00334: ;
    rdfs:comment "4 7  Slaughter establishments must have laboratory facility - Abrievated Graph Key: I95"@en-AU ;
    skos:definition "4 7  Slaughter establishments must have laboratory facility"@en-AU ;
    skos:narrower F2021L00334:88 ;
    skos:prefLabel "Item I95"@en-AU ;
    dcat:accessURL <https://www.legislation.gov.au/F2021L00334/2023-08-04/2023-08-04/text/original/epub/OEBPS/document_1/document_1.html#_Toc143507742> ;
    dcat:landingPage "https://www.legislation.gov.au/F2021L00334/2023-08-04/2023-08-04/text/original/epub/OEBPS/document_1/document_1.html#_Toc143507742"^^xsd:anyURI ;
    dcat:theme legcons:Item .

F2021L00334:96 a legcons:Item,
        owl:Class,
        dcat:Resource ;
    rdfs:label "Item - I96 4 8  Secure storage area"@en-AU ;
    dct:isPartOf F2021L00334:88 ;
    dct:isReferencedBy F2021L00334: ;
    rdfs:comment "4 8  Secure storage area - Abrievated Graph Key: I96"@en-AU ;
    skos:definition "4 8  Secure storage area"@en-AU ;
    skos:narrower F2021L00334:88 ;
    skos:prefLabel "Item I96"@en-AU ;
    dcat:accessURL <https://www.legislation.gov.au/F2021L00334/2023-08-04/2023-08-04/text/original/epub/OEBPS/document_1/document_1.html#_Toc143507743> ;
    dcat:landingPage "https://www.legislation.gov.au/F2021L00334/2023-08-04/2023-08-04/text/original/epub/OEBPS/document_1/document_1.html#_Toc143507743"^^xsd:anyURI ;
    dcat:theme legcons:Item .

F2021L00334:97 a legcons:Item,
        owl:Class,
        dcat:Resource ;
    rdfs:label "Item - I97 4 9  Amenities for Commonwealth authorised officers"@en-AU ;
    dct:isPartOf F2021L00334:88 ;
    dct:isReferencedBy F2021L00334: ;
    rdfs:comment "4 9  Amenities for Commonwealth authorised officers - Abrievated Graph Key: I97"@en-AU ;
    skos:definition "4 9  Amenities for Commonwealth authorised officers"@en-AU ;
    skos:narrower F2021L00334:88 ;
    skos:prefLabel "Item I97"@en-AU ;
    dcat:accessURL <https://www.legislation.gov.au/F2021L00334/2023-08-04/2023-08-04/text/original/epub/OEBPS/document_1/document_1.html#_Toc143507744> ;
    dcat:landingPage "https://www.legislation.gov.au/F2021L00334/2023-08-04/2023-08-04/text/original/epub/OEBPS/document_1/document_1.html#_Toc143507744"^^xsd:anyURI ;
    dcat:theme legcons:Item .

F2021L00334:99 a legcons:Item,
        owl:Class,
        dcat:Resource ;
    rdfs:label "Item - I99 4 10  Purpose of this Part"@en-AU ;
    dct:isPartOf F2021L00334:98 ;
    dct:isReferencedBy F2021L00334: ;
    rdfs:comment "4 10  Purpose of this Part - Abrievated Graph Key: I99"@en-AU ;
    skos:definition "4 10  Purpose of this Part"@en-AU ;
    skos:narrower F2021L00334:98 ;
    skos:prefLabel "Item I99"@en-AU ;
    dcat:accessURL <https://www.legislation.gov.au/F2021L00334/2023-08-04/2023-08-04/text/original/epub/OEBPS/document_1/document_1.html#_Toc143507746> ;
    dcat:landingPage "https://www.legislation.gov.au/F2021L00334/2023-08-04/2023-08-04/text/original/epub/OEBPS/document_1/document_1.html#_Toc143507746"^^xsd:anyURI ;
    dcat:theme legcons:Item .

F2021L00334:108 a legcons:Part,
        owl:Class,
        dcat:Resource ;
    rdfs:label "Part - P108 Part 4 Variation of registration"@en-AU ;
    dct:hasPart F2021L00334:109 ;
    dct:isPartOf F2021L00334:87 ;
    dct:isReferencedBy F2021L00334: ;
    rdfs:comment "Part 4 Variation of registration - Abrievated Graph Key: P108"@en-AU ;
    skos:broader F2021L00334:109 ;
    skos:definition "Part 4 Variation of registration"@en-AU ;
    skos:narrower F2021L00334:87 ;
    skos:prefLabel "Part P108"@en-AU ;
    dcat:accessURL <https://www.legislation.gov.au/F2021L00334/2023-08-04/2023-08-04/text/original/epub/OEBPS/document_1/document_1.html#_Toc143507755> ;
    dcat:landingPage "https://www.legislation.gov.au/F2021L00334/2023-08-04/2023-08-04/text/original/epub/OEBPS/document_1/document_1.html#_Toc143507755"^^xsd:anyURI ;
    dcat:theme legcons:Part .

F2021L00334:137 a legcons:Subdivision,
        owl:Class,
        dcat:Resource ;
    rdfs:label "Subdivision - S137 Subdivision APurpose of this Division"@en-AU ;
    dct:hasPart F2021L00334:138 ;
    dct:isPartOf F2021L00334:136 ;
    dct:isReferencedBy F2021L00334: ;
    rdfs:comment "Subdivision APurpose of this Division - Abrievated Graph Key: S137"@en-AU ;
    skos:broader F2021L00334:138 ;
    skos:definition "Subdivision APurpose of this Division"@en-AU ;
    skos:narrower F2021L00334:136 ;
    skos:prefLabel "Subdivision S137"@en-AU ;
    dcat:accessURL <https://www.legislation.gov.au/F2021L00334/2023-08-04/2023-08-04/text/original/epub/OEBPS/document_1/document_1.html#_Toc143507784> ;
    dcat:landingPage "https://www.legislation.gov.au/F2021L00334/2023-08-04/2023-08-04/text/original/epub/OEBPS/document_1/document_1.html#_Toc143507784"^^xsd:anyURI ;
    dcat:theme legcons:Subdivision .

F2021L00334:197 a legcons:Subdivision,
        owl:Class,
        dcat:Resource ;
    rdfs:label "Subdivision - S197 Subdivision BVariations required by Secretary"@en-AU ;
    dct:hasPart F2021L00334:198 ;
    dct:isPartOf F2021L00334:131 ;
    dct:isReferencedBy F2021L00334: ;
    rdfs:comment "Subdivision BVariations required by Secretary - Abrievated Graph Key: S197"@en-AU ;
    skos:broader F2021L00334:198 ;
    skos:definition "Subdivision BVariations required by Secretary"@en-AU ;
    skos:narrower F2021L00334:131 ;
    skos:prefLabel "Subdivision S197"@en-AU ;
    dcat:accessURL <https://www.legislation.gov.au/F2021L00334/2023-08-04/2023-08-04/text/original/epub/OEBPS/document_1/document_1.html#_Toc143507844> ;
    dcat:landingPage "https://www.legislation.gov.au/F2021L00334/2023-08-04/2023-08-04/text/original/epub/OEBPS/document_1/document_1.html#_Toc143507844"^^xsd:anyURI ;
    dcat:theme legcons:Subdivision .

F2021L00334:204 a legcons:Subdivision,
        owl:Class,
        dcat:Resource ;
    rdfs:label "Subdivision - S204 Subdivision APurpose of this Division"@en-AU ;
    dct:hasPart F2021L00334:205 ;
    dct:isPartOf F2021L00334:203 ;
    dct:isReferencedBy F2021L00334: ;
    rdfs:comment "Subdivision APurpose of this Division - Abrievated Graph Key: S204"@en-AU ;
    skos:broader F2021L00334:205 ;
    skos:definition "Subdivision APurpose of this Division"@en-AU ;
    skos:narrower F2021L00334:203 ;
    skos:prefLabel "Subdivision S204"@en-AU ;
    dcat:accessURL <https://www.legislation.gov.au/F2021L00334/2023-08-04/2023-08-04/text/original/epub/OEBPS/document_1/document_1.html#_Toc143507851> ;
    dcat:landingPage "https://www.legislation.gov.au/F2021L00334/2023-08-04/2023-08-04/text/original/epub/OEBPS/document_1/document_1.html#_Toc143507851"^^xsd:anyURI ;
    dcat:theme legcons:Subdivision .

F2021L00334:206 a legcons:Subdivision,
        owl:Class,
        dcat:Resource ;
    rdfs:label "Subdivision - S206 Subdivision BRequirements"@en-AU ;
    dct:hasPart F2021L00334:207 ;
    dct:isPartOf F2021L00334:203 ;
    dct:isReferencedBy F2021L00334: ;
    rdfs:comment "Subdivision BRequirements - Abrievated Graph Key: S206"@en-AU ;
    skos:broader F2021L00334:207 ;
    skos:definition "Subdivision BRequirements"@en-AU ;
    skos:narrower F2021L00334:203 ;
    skos:prefLabel "Subdivision S206"@en-AU ;
    dcat:accessURL <https://www.legislation.gov.au/F2021L00334/2023-08-04/2023-08-04/text/original/epub/OEBPS/document_1/document_1.html#_Toc143507853> ;
    dcat:landingPage "https://www.legislation.gov.au/F2021L00334/2023-08-04/2023-08-04/text/original/epub/OEBPS/document_1/document_1.html#_Toc143507853"^^xsd:anyURI ;
    dcat:theme legcons:Subdivision .

F2021L00334:215 a legcons:Division,
        owl:Class,
        dcat:Resource ;
    rdfs:label "Division - D215 Division 3 Renewal of approved arrangement"@en-AU ;
    dct:hasPart F2021L00334:216 ;
    dct:isPartOf F2021L00334:130 ;
    dct:isReferencedBy F2021L00334: ;
    rdfs:comment "Division 3 Renewal of approved arrangement - Abrievated Graph Key: D215"@en-AU ;
    skos:broader F2021L00334:216 ;
    skos:definition "Division 3 Renewal of approved arrangement"@en-AU ;
    skos:narrower F2021L00334:130 ;
    skos:prefLabel "Division D215"@en-AU ;
    dcat:accessURL <https://www.legislation.gov.au/F2021L00334/2023-08-04/2023-08-04/text/original/epub/OEBPS/document_1/document_1.html#_Toc143507862> ;
    dcat:landingPage "https://www.legislation.gov.au/F2021L00334/2023-08-04/2023-08-04/text/original/epub/OEBPS/document_1/document_1.html#_Toc143507862"^^xsd:anyURI ;
    dcat:theme legcons:Division .

F2021L00334:218 a legcons:Subdivision,
        owl:Class,
        dcat:Resource ;
    rdfs:label "Subdivision - S218 Subdivision AVariations by holder"@en-AU ;
    dct:hasPart F2021L00334:219 ;
    dct:isPartOf F2021L00334:217 ;
    dct:isReferencedBy F2021L00334: ;
    rdfs:comment "Subdivision AVariations by holder - Abrievated Graph Key: S218"@en-AU ;
    skos:broader F2021L00334:219 ;
    skos:definition "Subdivision AVariations by holder"@en-AU ;
    skos:narrower F2021L00334:217 ;
    skos:prefLabel "Subdivision S218"@en-AU ;
    dcat:accessURL <https://www.legislation.gov.au/F2021L00334/2023-08-04/2023-08-04/text/original/epub/OEBPS/document_1/document_1.html#_Toc143507865> ;
    dcat:landingPage "https://www.legislation.gov.au/F2021L00334/2023-08-04/2023-08-04/text/original/epub/OEBPS/document_1/document_1.html#_Toc143507865"^^xsd:anyURI ;
    dcat:theme legcons:Subdivision .

F2021L00334:220 a legcons:Subdivision,
        owl:Class,
        dcat:Resource ;
    rdfs:label "Subdivision - S220 Subdivision BVariations required by Secretary"@en-AU ;
    dct:hasPart F2021L00334:221 ;
    dct:isPartOf F2021L00334:217 ;
    dct:isReferencedBy F2021L00334: ;
    rdfs:comment "Subdivision BVariations required by Secretary - Abrievated Graph Key: S220"@en-AU ;
    skos:broader F2021L00334:221 ;
    skos:definition "Subdivision BVariations required by Secretary"@en-AU ;
    skos:narrower F2021L00334:217 ;
    skos:prefLabel "Subdivision S220"@en-AU ;
    dcat:accessURL <https://www.legislation.gov.au/F2021L00334/2023-08-04/2023-08-04/text/original/epub/OEBPS/document_1/document_1.html#_Toc143507867> ;
    dcat:landingPage "https://www.legislation.gov.au/F2021L00334/2023-08-04/2023-08-04/text/original/epub/OEBPS/document_1/document_1.html#_Toc143507867"^^xsd:anyURI ;
    dcat:theme legcons:Subdivision .

F2021L00334:222 a legcons:Division,
        owl:Class,
        dcat:Resource ;
    rdfs:label "Division - D222 Division 5 Obligations of holders of approved arrangements etc"@en-AU ;
    dct:hasPart F2021L00334:223 ;
    dct:isPartOf F2021L00334:130 ;
    dct:isReferencedBy F2021L00334: ;
    rdfs:comment "Division 5 Obligations of holders of approved arrangements etc - Abrievated Graph Key: D222"@en-AU ;
    skos:broader F2021L00334:223 ;
    skos:definition "Division 5 Obligations of holders of approved arrangements etc"@en-AU ;
    skos:narrower F2021L00334:130 ;
    skos:prefLabel "Division D222"@en-AU ;
    dcat:accessURL <https://www.legislation.gov.au/F2021L00334/2023-08-04/2023-08-04/text/original/epub/OEBPS/document_1/document_1.html#_Toc143507869> ;
    dcat:landingPage "https://www.legislation.gov.au/F2021L00334/2023-08-04/2023-08-04/text/original/epub/OEBPS/document_1/document_1.html#_Toc143507869"^^xsd:anyURI ;
    dcat:theme legcons:Division .

F2021L00334:224 a legcons:Division,
        owl:Class,
        dcat:Resource ;
    rdfs:label "Division - D224 Division 6 Fit and proper persons"@en-AU ;
    dct:hasPart F2021L00334:225 ;
    dct:isPartOf F2021L00334:130 ;
    dct:isReferencedBy F2021L00334: ;
    rdfs:comment "Division 6 Fit and proper persons - Abrievated Graph Key: D224"@en-AU ;
    skos:broader F2021L00334:225 ;
    skos:definition "Division 6 Fit and proper persons"@en-AU ;
    skos:narrower F2021L00334:130 ;
    skos:prefLabel "Division D224"@en-AU ;
    dcat:accessURL <https://www.legislation.gov.au/F2021L00334/2023-08-04/2023-08-04/text/original/epub/OEBPS/document_1/document_1.html#_Toc143507871> ;
    dcat:landingPage "https://www.legislation.gov.au/F2021L00334/2023-08-04/2023-08-04/text/original/epub/OEBPS/document_1/document_1.html#_Toc143507871"^^xsd:anyURI ;
    dcat:theme legcons:Division .

F2021L00334:232 a legcons:Part,
        owl:Class,
        dcat:Resource ;
    rdfs:label "Part - P232 Part 1 Requirements for grant of meat export licence"@en-AU ;
    dct:hasPart F2021L00334:233 ;
    dct:isPartOf F2021L00334:231 ;
    dct:isReferencedBy F2021L00334: ;
    rdfs:comment "Part 1 Requirements for grant of meat export licence - Abrievated Graph Key: P232"@en-AU ;
    skos:broader F2021L00334:233 ;
    skos:definition "Part 1 Requirements for grant of meat export licence"@en-AU ;
    skos:narrower F2021L00334:231 ;
    skos:prefLabel "Part P232"@en-AU ;
    dcat:accessURL <https://www.legislation.gov.au/F2021L00334/2023-08-04/2023-08-04/text/original/epub/OEBPS/document_1/document_1.html#_Toc143507879> ;
    dcat:landingPage "https://www.legislation.gov.au/F2021L00334/2023-08-04/2023-08-04/text/original/epub/OEBPS/document_1/document_1.html#_Toc143507879"^^xsd:anyURI ;
    dcat:theme legcons:Part .

F2021L00334:234 a legcons:Part,
        owl:Class,
        dcat:Resource ;
    rdfs:label "Part - P234 Part 2 Conditions of meat export licence"@en-AU ;
    dct:hasPart F2021L00334:235 ;
    dct:isPartOf F2021L00334:231 ;
    dct:isReferencedBy F2021L00334: ;
    rdfs:comment "Part 2 Conditions of meat export licence - Abrievated Graph Key: P234"@en-AU ;
    skos:broader F2021L00334:235 ;
    skos:definition "Part 2 Conditions of meat export licence"@en-AU ;
    skos:narrower F2021L00334:231 ;
    skos:prefLabel "Part P234"@en-AU ;
    dcat:accessURL <https://www.legislation.gov.au/F2021L00334/2023-08-04/2023-08-04/text/original/epub/OEBPS/document_1/document_1.html#_Toc143507881> ;
    dcat:landingPage "https://www.legislation.gov.au/F2021L00334/2023-08-04/2023-08-04/text/original/epub/OEBPS/document_1/document_1.html#_Toc143507881"^^xsd:anyURI ;
    dcat:theme legcons:Part .

F2021L00334:236 a legcons:Part,
        owl:Class,
        dcat:Resource ;
    rdfs:label "Part - P236 Part 3 Renewal of meat export licence"@en-AU ;
    dct:hasPart F2021L00334:237 ;
    dct:isPartOf F2021L00334:231 ;
    dct:isReferencedBy F2021L00334: ;
    rdfs:comment "Part 3 Renewal of meat export licence - Abrievated Graph Key: P236"@en-AU ;
    skos:broader F2021L00334:237 ;
    skos:definition "Part 3 Renewal of meat export licence"@en-AU ;
    skos:narrower F2021L00334:231 ;
    skos:prefLabel "Part P236"@en-AU ;
    dcat:accessURL <https://www.legislation.gov.au/F2021L00334/2023-08-04/2023-08-04/text/original/epub/OEBPS/document_1/document_1.html#_Toc143507883> ;
    dcat:landingPage "https://www.legislation.gov.au/F2021L00334/2023-08-04/2023-08-04/text/original/epub/OEBPS/document_1/document_1.html#_Toc143507883"^^xsd:anyURI ;
    dcat:theme legcons:Part .

F2021L00334:238 a legcons:Part,
        owl:Class,
        dcat:Resource ;
    rdfs:label "Part - P238 Part 4 Suspension of meat export licence"@en-AU ;
    dct:hasPart F2021L00334:239 ;
    dct:isPartOf F2021L00334:231 ;
    dct:isReferencedBy F2021L00334: ;
    rdfs:comment "Part 4 Suspension of meat export licence - Abrievated Graph Key: P238"@en-AU ;
    skos:broader F2021L00334:239 ;
    skos:definition "Part 4 Suspension of meat export licence"@en-AU ;
    skos:narrower F2021L00334:231 ;
    skos:prefLabel "Part P238"@en-AU ;
    dcat:accessURL <https://www.legislation.gov.au/F2021L00334/2023-08-04/2023-08-04/text/original/epub/OEBPS/document_1/document_1.html#_Toc143507885> ;
    dcat:landingPage "https://www.legislation.gov.au/F2021L00334/2023-08-04/2023-08-04/text/original/epub/OEBPS/document_1/document_1.html#_Toc143507885"^^xsd:anyURI ;
    dcat:theme legcons:Part .

F2021L00334:240 a legcons:Part,
        owl:Class,
        dcat:Resource ;
    rdfs:label "Part - P240 Part 5 Revocation of meat export licence"@en-AU ;
    dct:hasPart F2021L00334:241 ;
    dct:isPartOf F2021L00334:231 ;
    dct:isReferencedBy F2021L00334: ;
    rdfs:comment "Part 5 Revocation of meat export licence - Abrievated Graph Key: P240"@en-AU ;
    skos:broader F2021L00334:241 ;
    skos:definition "Part 5 Revocation of meat export licence"@en-AU ;
    skos:narrower F2021L00334:231 ;
    skos:prefLabel "Part P240"@en-AU ;
    dcat:accessURL <https://www.legislation.gov.au/F2021L00334/2023-08-04/2023-08-04/text/original/epub/OEBPS/document_1/document_1.html#_Toc143507887> ;
    dcat:landingPage "https://www.legislation.gov.au/F2021L00334/2023-08-04/2023-08-04/text/original/epub/OEBPS/document_1/document_1.html#_Toc143507887"^^xsd:anyURI ;
    dcat:theme legcons:Part .

F2021L00334:242 a legcons:Part,
        owl:Class,
        dcat:Resource ;
    rdfs:label "Part - P242 Part 6 Obligations of holders of meat export licences"@en-AU ;
    dct:hasPart F2021L00334:243 ;
    dct:isPartOf F2021L00334:231 ;
    dct:isReferencedBy F2021L00334: ;
    rdfs:comment "Part 6 Obligations of holders of meat export licences - Abrievated Graph Key: P242"@en-AU ;
    skos:broader F2021L00334:243 ;
    skos:definition "Part 6 Obligations of holders of meat export licences"@en-AU ;
    skos:narrower F2021L00334:231 ;
    skos:prefLabel "Part P242"@en-AU ;
    dcat:accessURL <https://www.legislation.gov.au/F2021L00334/2023-08-04/2023-08-04/text/original/epub/OEBPS/document_1/document_1.html#_Toc143507889> ;
    dcat:landingPage "https://www.legislation.gov.au/F2021L00334/2023-08-04/2023-08-04/text/original/epub/OEBPS/document_1/document_1.html#_Toc143507889"^^xsd:anyURI ;
    dcat:theme legcons:Part .

F2021L00334:244 a legcons:Part,
        owl:Class,
        dcat:Resource ;
    rdfs:label "Part - P244 Part 7 Fit and proper persons"@en-AU ;
    dct:hasPart F2021L00334:245 ;
    dct:isPartOf F2021L00334:231 ;
    dct:isReferencedBy F2021L00334: ;
    rdfs:comment "Part 7 Fit and proper persons - Abrievated Graph Key: P244"@en-AU ;
    skos:broader F2021L00334:245 ;
    skos:definition "Part 7 Fit and proper persons"@en-AU ;
    skos:narrower F2021L00334:231 ;
    skos:prefLabel "Part P244"@en-AU ;
    dcat:accessURL <https://www.legislation.gov.au/F2021L00334/2023-08-04/2023-08-04/text/original/epub/OEBPS/document_1/document_1.html#_Toc143507891> ;
    dcat:landingPage "https://www.legislation.gov.au/F2021L00334/2023-08-04/2023-08-04/text/original/epub/OEBPS/document_1/document_1.html#_Toc143507891"^^xsd:anyURI ;
    dcat:theme legcons:Part .

F2021L00334:252 a legcons:Part,
        owl:Class,
        dcat:Resource ;
    rdfs:label "Part - P252 Part 1 Issue of export permit"@en-AU ;
    dct:hasPart F2021L00334:253 ;
    dct:isPartOf F2021L00334:251 ;
    dct:isReferencedBy F2021L00334: ;
    rdfs:comment "Part 1 Issue of export permit - Abrievated Graph Key: P252"@en-AU ;
    skos:broader F2021L00334:253 ;
    skos:definition "Part 1 Issue of export permit"@en-AU ;
    skos:narrower F2021L00334:251 ;
    skos:prefLabel "Part P252"@en-AU ;
    dcat:accessURL <https://www.legislation.gov.au/F2021L00334/2023-08-04/2023-08-04/text/original/epub/OEBPS/document_1/document_1.html#_Toc143507899> ;
    dcat:landingPage "https://www.legislation.gov.au/F2021L00334/2023-08-04/2023-08-04/text/original/epub/OEBPS/document_1/document_1.html#_Toc143507899"^^xsd:anyURI ;
    dcat:theme legcons:Part .

F2021L00334:315 a legcons:Division,
        owl:Class,
        dcat:Resource ;
    rdfs:label "Division - D315 Division 1 General"@en-AU ;
    dct:hasPart F2021L00334:316 ;
    dct:isPartOf F2021L00334:314 ;
    dct:isReferencedBy F2021L00334: ;
    rdfs:comment "Division 1 General - Abrievated Graph Key: D315"@en-AU ;
    skos:broader F2021L00334:316 ;
    skos:definition "Division 1 General"@en-AU ;
    skos:narrower F2021L00334:314 ;
    skos:prefLabel "Division D315"@en-AU ;
    dcat:accessURL <https://www.legislation.gov.au/F2021L00334/2023-08-04/2023-08-04/text/original/epub/OEBPS/document_1/document_1.html#_Toc143507962> ;
    dcat:landingPage "https://www.legislation.gov.au/F2021L00334/2023-08-04/2023-08-04/text/original/epub/OEBPS/document_1/document_1.html#_Toc143507962"^^xsd:anyURI ;
    dcat:theme legcons:Division .

F2021L00334:334 a legcons:Part,
        owl:Class,
        dcat:Resource ;
    rdfs:label "Part - P334 Part 2 Assessments"@en-AU ;
    dct:hasPart F2021L00334:335 ;
    dct:isPartOf F2021L00334:313 ;
    dct:isReferencedBy F2021L00334: ;
    rdfs:comment "Part 2 Assessments - Abrievated Graph Key: P334"@en-AU ;
    skos:broader F2021L00334:335 ;
    skos:definition "Part 2 Assessments"@en-AU ;
    skos:narrower F2021L00334:313 ;
    skos:prefLabel "Part P334"@en-AU ;
    dcat:accessURL <https://www.legislation.gov.au/F2021L00334/2023-08-04/2023-08-04/text/original/epub/OEBPS/document_1/document_1.html#_Toc143507981> ;
    dcat:landingPage "https://www.legislation.gov.au/F2021L00334/2023-08-04/2023-08-04/text/original/epub/OEBPS/document_1/document_1.html#_Toc143507981"^^xsd:anyURI ;
    dcat:theme legcons:Part .

F2021L00334:336 a legcons:Part,
        owl:Class,
        dcat:Resource ;
    rdfs:label "Part - P336 Part 3 Powers of the Secretary"@en-AU ;
    dct:hasPart F2021L00334:337 ;
    dct:isPartOf F2021L00334:313 ;
    dct:isReferencedBy F2021L00334: ;
    rdfs:comment "Part 3 Powers of the Secretary - Abrievated Graph Key: P336"@en-AU ;
    skos:broader F2021L00334:337 ;
    skos:definition "Part 3 Powers of the Secretary"@en-AU ;
    skos:narrower F2021L00334:313 ;
    skos:prefLabel "Part P336"@en-AU ;
    dcat:accessURL <https://www.legislation.gov.au/F2021L00334/2023-08-04/2023-08-04/text/original/epub/OEBPS/document_1/document_1.html#_Toc143507983> ;
    dcat:landingPage "https://www.legislation.gov.au/F2021L00334/2023-08-04/2023-08-04/text/original/epub/OEBPS/document_1/document_1.html#_Toc143507983"^^xsd:anyURI ;
    dcat:theme legcons:Part .

F2021L00334:339 a legcons:Division,
        owl:Class,
        dcat:Resource ;
    rdfs:label "Division - D339 Division 1 Third party authorised officers"@en-AU ;
    dct:hasPart F2021L00334:340 ;
    dct:isPartOf F2021L00334:338 ;
    dct:isReferencedBy F2021L00334: ;
    rdfs:comment "Division 1 Third party authorised officers - Abrievated Graph Key: D339"@en-AU ;
    skos:broader F2021L00334:340 ;
    skos:definition "Division 1 Third party authorised officers"@en-AU ;
    skos:narrower F2021L00334:338 ;
    skos:prefLabel "Division D339"@en-AU ;
    dcat:accessURL <https://www.legislation.gov.au/F2021L00334/2023-08-04/2023-08-04/text/original/epub/OEBPS/document_1/document_1.html#_Toc143507986> ;
    dcat:landingPage "https://www.legislation.gov.au/F2021L00334/2023-08-04/2023-08-04/text/original/epub/OEBPS/document_1/document_1.html#_Toc143507986"^^xsd:anyURI ;
    dcat:theme legcons:Division .

F2021L00334:356 a legcons:Division,
        owl:Class,
        dcat:Resource ;
    rdfs:label "Division - D356 Division 3 Directions to deal with non compliance with the Act etc"@en-AU ;
    dct:hasPart F2021L00334:357 ;
    dct:isPartOf F2021L00334:338 ;
    dct:isReferencedBy F2021L00334: ;
    rdfs:comment "Division 3 Directions to deal with non compliance with the Act etc - Abrievated Graph Key: D356"@en-AU ;
    skos:broader F2021L00334:357 ;
    skos:definition "Division 3 Directions to deal with non compliance with the Act etc"@en-AU ;
    skos:narrower F2021L00334:338 ;
    skos:prefLabel "Division D356"@en-AU ;
    dcat:accessURL <https://www.legislation.gov.au/F2021L00334/2023-08-04/2023-08-04/text/original/epub/OEBPS/document_1/document_1.html#_Toc143508003> ;
    dcat:landingPage "https://www.legislation.gov.au/F2021L00334/2023-08-04/2023-08-04/text/original/epub/OEBPS/document_1/document_1.html#_Toc143508003"^^xsd:anyURI ;
    dcat:theme legcons:Division .

F2021L00334:358 a legcons:Division,
        owl:Class,
        dcat:Resource ;
    rdfs:label "Division - D358 Division 4 Miscellaneous"@en-AU ;
    dct:hasPart F2021L00334:359 ;
    dct:isPartOf F2021L00334:338 ;
    dct:isReferencedBy F2021L00334: ;
    rdfs:comment "Division 4 Miscellaneous - Abrievated Graph Key: D358"@en-AU ;
    skos:broader F2021L00334:359 ;
    skos:definition "Division 4 Miscellaneous"@en-AU ;
    skos:narrower F2021L00334:338 ;
    skos:prefLabel "Division D358"@en-AU ;
    dcat:accessURL <https://www.legislation.gov.au/F2021L00334/2023-08-04/2023-08-04/text/original/epub/OEBPS/document_1/document_1.html#_Toc143508005> ;
    dcat:landingPage "https://www.legislation.gov.au/F2021L00334/2023-08-04/2023-08-04/text/original/epub/OEBPS/document_1/document_1.html#_Toc143508005"^^xsd:anyURI ;
    dcat:theme legcons:Division .

F2021L00334:360 a legcons:Chapter,
        owl:Class,
        dcat:Resource ;
    rdfs:label "Chapter - C360 Chapter 10 Compliance and enforcement"@en-AU ;
    dct:hasPart F2021L00334:361,
        F2021L00334:362 ;
    dct:isReferencedBy F2021L00334: ;
    rdfs:comment "Chapter 10 Compliance and enforcement - Abrievated Graph Key: C360"@en-AU ;
    skos:broader F2021L00334:361,
        F2021L00334:362 ;
    skos:definition "Chapter 10 Compliance and enforcement"@en-AU ;
    skos:prefLabel "Chapter C360"@en-AU ;
    dcat:accessURL <https://www.legislation.gov.au/F2021L00334/2023-08-04/2023-08-04/text/original/epub/OEBPS/document_1/document_1.html#_Toc143508007> ;
    dcat:landingPage "https://www.legislation.gov.au/F2021L00334/2023-08-04/2023-08-04/text/original/epub/OEBPS/document_1/document_1.html#_Toc143508007"^^xsd:anyURI ;
    dcat:theme legcons:Chapter .

F2021L00334:364 a legcons:Part,
        owl:Class,
        dcat:Resource ;
    rdfs:label "Part - P364 Part 1 Review of decisions"@en-AU ;
    dct:hasPart F2021L00334:365 ;
    dct:isPartOf F2021L00334:363 ;
    dct:isReferencedBy F2021L00334: ;
    rdfs:comment "Part 1 Review of decisions - Abrievated Graph Key: P364"@en-AU ;
    skos:broader F2021L00334:365 ;
    skos:definition "Part 1 Review of decisions"@en-AU ;
    skos:narrower F2021L00334:363 ;
    skos:prefLabel "Part P364"@en-AU ;
    dcat:accessURL <https://www.legislation.gov.au/F2021L00334/2023-08-04/2023-08-04/text/original/epub/OEBPS/document_1/document_1.html#_Toc143508011> ;
    dcat:landingPage "https://www.legislation.gov.au/F2021L00334/2023-08-04/2023-08-04/text/original/epub/OEBPS/document_1/document_1.html#_Toc143508011"^^xsd:anyURI ;
    dcat:theme legcons:Part .

F2021L00334:378 a legcons:Part,
        owl:Class,
        dcat:Resource ;
    rdfs:label "Part - P378 Part 3 Samples"@en-AU ;
    dct:hasPart F2021L00334:379 ;
    dct:isPartOf F2021L00334:363 ;
    dct:isReferencedBy F2021L00334: ;
    rdfs:comment "Part 3 Samples - Abrievated Graph Key: P378"@en-AU ;
    skos:broader F2021L00334:379 ;
    skos:definition "Part 3 Samples"@en-AU ;
    skos:narrower F2021L00334:363 ;
    skos:prefLabel "Part P378"@en-AU ;
    dcat:accessURL <https://www.legislation.gov.au/F2021L00334/2023-08-04/2023-08-04/text/original/epub/OEBPS/document_1/document_1.html#_Toc143508025> ;
    dcat:landingPage "https://www.legislation.gov.au/F2021L00334/2023-08-04/2023-08-04/text/original/epub/OEBPS/document_1/document_1.html#_Toc143508025"^^xsd:anyURI ;
    dcat:theme legcons:Part .

F2021L00334:383 a legcons:Part,
        owl:Class,
        dcat:Resource ;
    rdfs:label "Part - P383 Part 5 Relevant Commonwealth liabilities"@en-AU ;
    dct:hasPart F2021L00334:384 ;
    dct:isPartOf F2021L00334:363 ;
    dct:isReferencedBy F2021L00334: ;
    rdfs:comment "Part 5 Relevant Commonwealth liabilities - Abrievated Graph Key: P383"@en-AU ;
    skos:broader F2021L00334:384 ;
    skos:definition "Part 5 Relevant Commonwealth liabilities"@en-AU ;
    skos:narrower F2021L00334:363 ;
    skos:prefLabel "Part P383"@en-AU ;
    dcat:accessURL <https://www.legislation.gov.au/F2021L00334/2023-08-04/2023-08-04/text/original/epub/OEBPS/document_1/document_1.html#_Toc143508030> ;
    dcat:landingPage "https://www.legislation.gov.au/F2021L00334/2023-08-04/2023-08-04/text/original/epub/OEBPS/document_1/document_1.html#_Toc143508030"^^xsd:anyURI ;
    dcat:theme legcons:Part .

F2021L00334:386 a legcons:Part,
        owl:Class,
        dcat:Resource ;
    rdfs:label "Part - P386 Part 1 Preliminary"@en-AU ;
    dct:hasPart F2021L00334:387 ;
    dct:isPartOf F2021L00334:385 ;
    dct:isReferencedBy F2021L00334: ;
    rdfs:comment "Part 1 Preliminary - Abrievated Graph Key: P386"@en-AU ;
    skos:broader F2021L00334:387 ;
    skos:definition "Part 1 Preliminary"@en-AU ;
    skos:narrower F2021L00334:385 ;
    skos:prefLabel "Part P386"@en-AU ;
    dcat:accessURL <https://www.legislation.gov.au/F2021L00334/2023-08-04/2023-08-04/text/original/epub/OEBPS/document_1/document_1.html#_Toc143508033> ;
    dcat:landingPage "https://www.legislation.gov.au/F2021L00334/2023-08-04/2023-08-04/text/original/epub/OEBPS/document_1/document_1.html#_Toc143508033"^^xsd:anyURI ;
    dcat:theme legcons:Part .

F2021L00334:406 a legcons:Part,
        owl:Class,
        dcat:Resource ;
    rdfs:label "Part - P406 Part 3 Approved arrangements"@en-AU ;
    dct:hasPart F2021L00334:407 ;
    dct:isPartOf F2021L00334:385 ;
    dct:isReferencedBy F2021L00334: ;
    rdfs:comment "Part 3 Approved arrangements - Abrievated Graph Key: P406"@en-AU ;
    skos:broader F2021L00334:407 ;
    skos:definition "Part 3 Approved arrangements"@en-AU ;
    skos:narrower F2021L00334:385 ;
    skos:prefLabel "Part P406"@en-AU ;
    dcat:accessURL <https://www.legislation.gov.au/F2021L00334/2023-08-04/2023-08-04/text/original/epub/OEBPS/document_1/document_1.html#_Toc143508053> ;
    dcat:landingPage "https://www.legislation.gov.au/F2021L00334/2023-08-04/2023-08-04/text/original/epub/OEBPS/document_1/document_1.html#_Toc143508053"^^xsd:anyURI ;
    dcat:theme legcons:Part .

F2021L00334:409 a legcons:Division,
        owl:Class,
        dcat:Resource ;
    rdfs:label "Division - D409 Division 1 Trade descriptions"@en-AU ;
    dct:hasPart F2021L00334:410 ;
    dct:isPartOf F2021L00334:408 ;
    dct:isReferencedBy F2021L00334: ;
    rdfs:comment "Division 1 Trade descriptions - Abrievated Graph Key: D409"@en-AU ;
    skos:broader F2021L00334:410 ;
    skos:definition "Division 1 Trade descriptions"@en-AU ;
    skos:narrower F2021L00334:408 ;
    skos:prefLabel "Division D409"@en-AU ;
    dcat:accessURL <https://www.legislation.gov.au/F2021L00334/2023-08-04/2023-08-04/text/original/epub/OEBPS/document_1/document_1.html#_Toc143508056> ;
    dcat:landingPage "https://www.legislation.gov.au/F2021L00334/2023-08-04/2023-08-04/text/original/epub/OEBPS/document_1/document_1.html#_Toc143508056"^^xsd:anyURI ;
    dcat:theme legcons:Division .

F2021L00334:77 a legcons:Part,
        owl:Class,
        dcat:Resource ;
    rdfs:label "Part - P77 Part 6 Revocation of accreditation"@en-AU ;
    dct:hasPart F2021L00334:78 ;
    dct:isPartOf F2021L00334:37 ;
    dct:isReferencedBy F2021L00334: ;
    rdfs:comment "Part 6 Revocation of accreditation - Abrievated Graph Key: P77"@en-AU ;
    skos:broader F2021L00334:78 ;
    skos:definition "Part 6 Revocation of accreditation"@en-AU ;
    skos:narrower F2021L00334:37 ;
    skos:prefLabel "Part P77"@en-AU ;
    dcat:accessURL <https://www.legislation.gov.au/F2021L00334/2023-08-04/2023-08-04/text/original/epub/OEBPS/document_1/document_1.html#_Toc143507724> ;
    dcat:landingPage "https://www.legislation.gov.au/F2021L00334/2023-08-04/2023-08-04/text/original/epub/OEBPS/document_1/document_1.html#_Toc143507724"^^xsd:anyURI ;
    dcat:theme legcons:Part .

F2021L00334:105 a legcons:Part,
        owl:Class,
        dcat:Resource ;
    rdfs:label "Part - P105 Part 3 Renewal of registration"@en-AU ;
    dct:hasPart F2021L00334:106,
        F2021L00334:107 ;
    dct:isPartOf F2021L00334:87 ;
    dct:isReferencedBy F2021L00334: ;
    rdfs:comment "Part 3 Renewal of registration - Abrievated Graph Key: P105"@en-AU ;
    skos:broader F2021L00334:106,
        F2021L00334:107 ;
    skos:definition "Part 3 Renewal of registration"@en-AU ;
    skos:narrower F2021L00334:87 ;
    skos:prefLabel "Part P105"@en-AU ;
    dcat:accessURL <https://www.legislation.gov.au/F2021L00334/2023-08-04/2023-08-04/text/original/epub/OEBPS/document_1/document_1.html#_Toc143507752> ;
    dcat:landingPage "https://www.legislation.gov.au/F2021L00334/2023-08-04/2023-08-04/text/original/epub/OEBPS/document_1/document_1.html#_Toc143507752"^^xsd:anyURI ;
    dcat:theme legcons:Part .

F2021L00334:114 a legcons:Part,
        owl:Class,
        dcat:Resource ;
    rdfs:label "Part - P114 Part 6 Meat inspection services"@en-AU ;
    dct:hasPart F2021L00334:115,
        F2021L00334:124 ;
    dct:isPartOf F2021L00334:87 ;
    dct:isReferencedBy F2021L00334: ;
    rdfs:comment "Part 6 Meat inspection services - Abrievated Graph Key: P114"@en-AU ;
    skos:broader F2021L00334:115,
        F2021L00334:124 ;
    skos:definition "Part 6 Meat inspection services"@en-AU ;
    skos:narrower F2021L00334:87 ;
    skos:prefLabel "Part P114"@en-AU ;
    dcat:accessURL <https://www.legislation.gov.au/F2021L00334/2023-08-04/2023-08-04/text/original/epub/OEBPS/document_1/document_1.html#_Toc143507761> ;
    dcat:landingPage "https://www.legislation.gov.au/F2021L00334/2023-08-04/2023-08-04/text/original/epub/OEBPS/document_1/document_1.html#_Toc143507761"^^xsd:anyURI ;
    dcat:theme legcons:Part .

F2021L00334:14 a legcons:Chapter,
        owl:Class,
        dcat:Resource ;
    rdfs:label "Chapter - C14 Chapter 2 Exporting goods"@en-AU ;
    dct:hasPart F2021L00334:15,
        F2021L00334:22,
        F2021L00334:29 ;
    dct:isReferencedBy F2021L00334: ;
    rdfs:comment "Chapter 2 Exporting goods - Abrievated Graph Key: C14"@en-AU ;
    skos:broader F2021L00334:15,
        F2021L00334:22,
        F2021L00334:29 ;
    skos:definition "Chapter 2 Exporting goods"@en-AU ;
    skos:prefLabel "Chapter C14"@en-AU ;
    dcat:accessURL <https://www.legislation.gov.au/F2021L00334/2023-08-04/2023-08-04/text/original/epub/OEBPS/document_1/document_1.html#_Toc143507661> ;
    dcat:landingPage "https://www.legislation.gov.au/F2021L00334/2023-08-04/2023-08-04/text/original/epub/OEBPS/document_1/document_1.html#_Toc143507661"^^xsd:anyURI ;
    dcat:theme legcons:Chapter .

F2021L00334:15 a legcons:Part,
        owl:Class,
        dcat:Resource ;
    rdfs:label "Part - P15 Part 1 Goods"@en-AU ;
    dct:hasPart F2021L00334:16,
        F2021L00334:19 ;
    dct:isPartOf F2021L00334:14 ;
    dct:isReferencedBy F2021L00334: ;
    rdfs:comment "Part 1 Goods - Abrievated Graph Key: P15"@en-AU ;
    skos:broader F2021L00334:16,
        F2021L00334:19 ;
    skos:definition "Part 1 Goods"@en-AU ;
    skos:narrower F2021L00334:14 ;
    skos:prefLabel "Part P15"@en-AU ;
    dcat:accessURL <https://www.legislation.gov.au/F2021L00334/2023-08-04/2023-08-04/text/original/epub/OEBPS/document_1/document_1.html#_Toc143507662> ;
    dcat:landingPage "https://www.legislation.gov.au/F2021L00334/2023-08-04/2023-08-04/text/original/epub/OEBPS/document_1/document_1.html#_Toc143507662"^^xsd:anyURI ;
    dcat:theme legcons:Part .

F2021L00334:16 a legcons:Division,
        owl:Class,
        dcat:Resource ;
    rdfs:label "Division - D16 Division 1 Prescribed goods"@en-AU ;
    dct:hasPart F2021L00334:17,
        F2021L00334:18 ;
    dct:isPartOf F2021L00334:15 ;
    dct:isReferencedBy F2021L00334: ;
    rdfs:comment "Division 1 Prescribed goods - Abrievated Graph Key: D16"@en-AU ;
    skos:broader F2021L00334:17,
        F2021L00334:18 ;
    skos:definition "Division 1 Prescribed goods"@en-AU ;
    skos:narrower F2021L00334:15 ;
    skos:prefLabel "Division D16"@en-AU ;
    dcat:accessURL <https://www.legislation.gov.au/F2021L00334/2023-08-04/2023-08-04/text/original/epub/OEBPS/document_1/document_1.html#_Toc143507663> ;
    dcat:landingPage "https://www.legislation.gov.au/F2021L00334/2023-08-04/2023-08-04/text/original/epub/OEBPS/document_1/document_1.html#_Toc143507663"^^xsd:anyURI ;
    dcat:theme legcons:Division .

F2021L00334:19 a legcons:Division,
        owl:Class,
        dcat:Resource ;
    rdfs:label "Division - D19 Division 2 Prohibited export and prescribed export conditions"@en-AU ;
    dct:hasPart F2021L00334:20,
        F2021L00334:21 ;
    dct:isPartOf F2021L00334:15 ;
    dct:isReferencedBy F2021L00334: ;
    rdfs:comment "Division 2 Prohibited export and prescribed export conditions - Abrievated Graph Key: D19"@en-AU ;
    skos:broader F2021L00334:20,
        F2021L00334:21 ;
    skos:definition "Division 2 Prohibited export and prescribed export conditions"@en-AU ;
    skos:narrower F2021L00334:15 ;
    skos:prefLabel "Division D19"@en-AU ;
    dcat:accessURL <https://www.legislation.gov.au/F2021L00334/2023-08-04/2023-08-04/text/original/epub/OEBPS/document_1/document_1.html#_Toc143507666> ;
    dcat:landingPage "https://www.legislation.gov.au/F2021L00334/2023-08-04/2023-08-04/text/original/epub/OEBPS/document_1/document_1.html#_Toc143507666"^^xsd:anyURI ;
    dcat:theme legcons:Division .

F2021L00334:194 a legcons:Subdivision,
        owl:Class,
        dcat:Resource ;
    rdfs:label "Subdivision - S194 Subdivision AVariations by holder"@en-AU ;
    dct:hasPart F2021L00334:195,
        F2021L00334:196 ;
    dct:isPartOf F2021L00334:131 ;
    dct:isReferencedBy F2021L00334: ;
    rdfs:comment "Subdivision AVariations by holder - Abrievated Graph Key: S194"@en-AU ;
    skos:broader F2021L00334:195,
        F2021L00334:196 ;
    skos:definition "Subdivision AVariations by holder"@en-AU ;
    skos:narrower F2021L00334:131 ;
    skos:prefLabel "Subdivision S194"@en-AU ;
    dcat:accessURL <https://www.legislation.gov.au/F2021L00334/2023-08-04/2023-08-04/text/original/epub/OEBPS/document_1/document_1.html#_Toc143507841> ;
    dcat:landingPage "https://www.legislation.gov.au/F2021L00334/2023-08-04/2023-08-04/text/original/epub/OEBPS/document_1/document_1.html#_Toc143507841"^^xsd:anyURI ;
    dcat:theme legcons:Subdivision .

F2021L00334:200 a legcons:Division,
        owl:Class,
        dcat:Resource ;
    rdfs:label "Division - D200 Division 1 Requirements for approval"@en-AU ;
    dct:hasPart F2021L00334:201,
        F2021L00334:202 ;
    dct:isPartOf F2021L00334:130 ;
    dct:isReferencedBy F2021L00334: ;
    rdfs:comment "Division 1 Requirements for approval - Abrievated Graph Key: D200"@en-AU ;
    skos:broader F2021L00334:201,
        F2021L00334:202 ;
    skos:definition "Division 1 Requirements for approval"@en-AU ;
    skos:narrower F2021L00334:130 ;
    skos:prefLabel "Division D200"@en-AU ;
    dcat:accessURL <https://www.legislation.gov.au/F2021L00334/2023-08-04/2023-08-04/text/original/epub/OEBPS/document_1/document_1.html#_Toc143507847> ;
    dcat:landingPage "https://www.legislation.gov.au/F2021L00334/2023-08-04/2023-08-04/text/original/epub/OEBPS/document_1/document_1.html#_Toc143507847"^^xsd:anyURI ;
    dcat:theme legcons:Division .

F2021L00334:217 a legcons:Division,
        owl:Class,
        dcat:Resource ;
    rdfs:label "Division - D217 Division 4 Variation of approved arrangement"@en-AU ;
    dct:hasPart F2021L00334:218,
        F2021L00334:220 ;
    dct:isPartOf F2021L00334:130 ;
    dct:isReferencedBy F2021L00334: ;
    rdfs:comment "Division 4 Variation of approved arrangement - Abrievated Graph Key: D217"@en-AU ;
    skos:broader F2021L00334:218,
        F2021L00334:220 ;
    skos:definition "Division 4 Variation of approved arrangement"@en-AU ;
    skos:narrower F2021L00334:130 ;
    skos:prefLabel "Division D217"@en-AU ;
    dcat:accessURL <https://www.legislation.gov.au/F2021L00334/2023-08-04/2023-08-04/text/original/epub/OEBPS/document_1/document_1.html#_Toc143507864> ;
    dcat:landingPage "https://www.legislation.gov.au/F2021L00334/2023-08-04/2023-08-04/text/original/epub/OEBPS/document_1/document_1.html#_Toc143507864"^^xsd:anyURI ;
    dcat:theme legcons:Division .

F2021L00334:251 a legcons:Chapter,
        owl:Class,
        dcat:Resource ;
    rdfs:label "Chapter - C251 Chapter 7 Export permits"@en-AU ;
    dct:hasPart F2021L00334:252,
        F2021L00334:254,
        F2021L00334:258 ;
    dct:isReferencedBy F2021L00334: ;
    rdfs:comment "Chapter 7 Export permits - Abrievated Graph Key: C251"@en-AU ;
    skos:broader F2021L00334:252,
        F2021L00334:254,
        F2021L00334:258 ;
    skos:definition "Chapter 7 Export permits"@en-AU ;
    skos:prefLabel "Chapter C251"@en-AU ;
    dcat:accessURL <https://www.legislation.gov.au/F2021L00334/2023-08-04/2023-08-04/text/original/epub/OEBPS/document_1/document_1.html#_Toc143507898> ;
    dcat:landingPage "https://www.legislation.gov.au/F2021L00334/2023-08-04/2023-08-04/text/original/epub/OEBPS/document_1/document_1.html#_Toc143507898"^^xsd:anyURI ;
    dcat:theme legcons:Chapter .

F2021L00334:263 a legcons:Chapter,
        owl:Class,
        dcat:Resource ;
    rdfs:label "Chapter - C263 Chapter 8 Other matters relating to export"@en-AU ;
    dct:hasPart F2021L00334:264,
        F2021L00334:269,
        F2021L00334:273 ;
    dct:isReferencedBy F2021L00334: ;
    rdfs:comment "Chapter 8 Other matters relating to export - Abrievated Graph Key: C263"@en-AU ;
    skos:broader F2021L00334:264,
        F2021L00334:269,
        F2021L00334:273 ;
    skos:definition "Chapter 8 Other matters relating to export"@en-AU ;
    skos:prefLabel "Chapter C263"@en-AU ;
    dcat:accessURL <https://www.legislation.gov.au/F2021L00334/2023-08-04/2023-08-04/text/original/epub/OEBPS/document_1/document_1.html#_Toc143507910> ;
    dcat:landingPage "https://www.legislation.gov.au/F2021L00334/2023-08-04/2023-08-04/text/original/epub/OEBPS/document_1/document_1.html#_Toc143507910"^^xsd:anyURI ;
    dcat:theme legcons:Chapter .

F2021L00334:38 a legcons:Part,
        owl:Class,
        dcat:Resource ;
    rdfs:label "Part - P38 Part 1 Introduction"@en-AU ;
    dct:hasPart F2021L00334:39,
        F2021L00334:40 ;
    dct:isPartOf F2021L00334:37 ;
    dct:isReferencedBy F2021L00334: ;
    rdfs:comment "Part 1 Introduction - Abrievated Graph Key: P38"@en-AU ;
    skos:broader F2021L00334:39,
        F2021L00334:40 ;
    skos:definition "Part 1 Introduction"@en-AU ;
    skos:narrower F2021L00334:37 ;
    skos:prefLabel "Part P38"@en-AU ;
    dcat:accessURL <https://www.legislation.gov.au/F2021L00334/2023-08-04/2023-08-04/text/original/epub/OEBPS/document_1/document_1.html#_Toc143507685> ;
    dcat:landingPage "https://www.legislation.gov.au/F2021L00334/2023-08-04/2023-08-04/text/original/epub/OEBPS/document_1/document_1.html#_Toc143507685"^^xsd:anyURI ;
    dcat:theme legcons:Part .

F2021L00334:380 a legcons:Part,
        owl:Class,
        dcat:Resource ;
    rdfs:label "Part - P380 Part 4 Damaged or destroyed meat or meat products"@en-AU ;
    dct:hasPart F2021L00334:381,
        F2021L00334:382 ;
    dct:isPartOf F2021L00334:363 ;
    dct:isReferencedBy F2021L00334: ;
    rdfs:comment "Part 4 Damaged or destroyed meat or meat products - Abrievated Graph Key: P380"@en-AU ;
    skos:broader F2021L00334:381,
        F2021L00334:382 ;
    skos:definition "Part 4 Damaged or destroyed meat or meat products"@en-AU ;
    skos:narrower F2021L00334:363 ;
    skos:prefLabel "Part P380"@en-AU ;
    dcat:accessURL <https://www.legislation.gov.au/F2021L00334/2023-08-04/2023-08-04/text/original/epub/OEBPS/document_1/document_1.html#_Toc143508027> ;
    dcat:landingPage "https://www.legislation.gov.au/F2021L00334/2023-08-04/2023-08-04/text/original/epub/OEBPS/document_1/document_1.html#_Toc143508027"^^xsd:anyURI ;
    dcat:theme legcons:Part .

F2021L00334:41 a legcons:Part,
        owl:Class,
        dcat:Resource ;
    rdfs:label "Part - P41 Part 2 Requirements for accreditation etc"@en-AU ;
    dct:hasPart F2021L00334:42,
        F2021L00334:47 ;
    dct:isPartOf F2021L00334:37 ;
    dct:isReferencedBy F2021L00334: ;
    rdfs:comment "Part 2 Requirements for accreditation etc - Abrievated Graph Key: P41"@en-AU ;
    skos:broader F2021L00334:42,
        F2021L00334:47 ;
    skos:definition "Part 2 Requirements for accreditation etc"@en-AU ;
    skos:narrower F2021L00334:37 ;
    skos:prefLabel "Part P41"@en-AU ;
    dcat:accessURL <https://www.legislation.gov.au/F2021L00334/2023-08-04/2023-08-04/text/original/epub/OEBPS/document_1/document_1.html#_Toc143507688> ;
    dcat:landingPage "https://www.legislation.gov.au/F2021L00334/2023-08-04/2023-08-04/text/original/epub/OEBPS/document_1/document_1.html#_Toc143507688"^^xsd:anyURI ;
    dcat:theme legcons:Part .

F2021L00334:415 a legcons:Division,
        owl:Class,
        dcat:Resource ;
    rdfs:label "Division - D415 Division 3 Official marking devices"@en-AU ;
    dct:hasPart F2021L00334:416,
        F2021L00334:417 ;
    dct:isPartOf F2021L00334:408 ;
    dct:isReferencedBy F2021L00334: ;
    rdfs:comment "Division 3 Official marking devices - Abrievated Graph Key: D415"@en-AU ;
    skos:broader F2021L00334:416,
        F2021L00334:417 ;
    skos:definition "Division 3 Official marking devices"@en-AU ;
    skos:narrower F2021L00334:408 ;
    skos:prefLabel "Division D415"@en-AU ;
    dcat:accessURL <https://www.legislation.gov.au/F2021L00334/2023-08-04/2023-08-04/text/original/epub/OEBPS/document_1/document_1.html#_Toc143508062> ;
    dcat:landingPage "https://www.legislation.gov.au/F2021L00334/2023-08-04/2023-08-04/text/original/epub/OEBPS/document_1/document_1.html#_Toc143508062"^^xsd:anyURI ;
    dcat:theme legcons:Division .

F2021L00334:418 a legcons:Part,
        owl:Class,
        dcat:Resource ;
    rdfs:label "Part - P418 Part 5 Powers and officials"@en-AU ;
    dct:hasPart F2021L00334:419,
        F2021L00334:423 ;
    dct:isPartOf F2021L00334:385 ;
    dct:isReferencedBy F2021L00334: ;
    rdfs:comment "Part 5 Powers and officials - Abrievated Graph Key: P418"@en-AU ;
    skos:broader F2021L00334:419,
        F2021L00334:423 ;
    skos:definition "Part 5 Powers and officials"@en-AU ;
    skos:narrower F2021L00334:385 ;
    skos:prefLabel "Part P418"@en-AU ;
    dcat:accessURL <https://www.legislation.gov.au/F2021L00334/2023-08-04/2023-08-04/text/original/epub/OEBPS/document_1/document_1.html#_Toc143508065> ;
    dcat:landingPage "https://www.legislation.gov.au/F2021L00334/2023-08-04/2023-08-04/text/original/epub/OEBPS/document_1/document_1.html#_Toc143508065"^^xsd:anyURI ;
    dcat:theme legcons:Part .

F2021L00334:47 a legcons:Division,
        owl:Class,
        dcat:Resource ;
    rdfs:label "Division - D47 Division 2 Other matters relating to accreditation"@en-AU ;
    dct:hasPart F2021L00334:48,
        F2021L00334:49 ;
    dct:isPartOf F2021L00334:41 ;
    dct:isReferencedBy F2021L00334: ;
    rdfs:comment "Division 2 Other matters relating to accreditation - Abrievated Graph Key: D47"@en-AU ;
    skos:broader F2021L00334:48,
        F2021L00334:49 ;
    skos:definition "Division 2 Other matters relating to accreditation"@en-AU ;
    skos:narrower F2021L00334:41 ;
    skos:prefLabel "Division D47"@en-AU ;
    dcat:accessURL <https://www.legislation.gov.au/F2021L00334/2023-08-04/2023-08-04/text/original/epub/OEBPS/document_1/document_1.html#_Toc143507694> ;
    dcat:landingPage "https://www.legislation.gov.au/F2021L00334/2023-08-04/2023-08-04/text/original/epub/OEBPS/document_1/document_1.html#_Toc143507694"^^xsd:anyURI ;
    dcat:theme legcons:Division .

F2021L00334:71 a legcons:Part,
        owl:Class,
        dcat:Resource ;
    rdfs:label "Part - P71 Part 4 Renewal of accreditation"@en-AU ;
    dct:hasPart F2021L00334:72,
        F2021L00334:73 ;
    dct:isPartOf F2021L00334:37 ;
    dct:isReferencedBy F2021L00334: ;
    rdfs:comment "Part 4 Renewal of accreditation - Abrievated Graph Key: P71"@en-AU ;
    skos:broader F2021L00334:72,
        F2021L00334:73 ;
    skos:definition "Part 4 Renewal of accreditation"@en-AU ;
    skos:narrower F2021L00334:37 ;
    skos:prefLabel "Part P71"@en-AU ;
    dcat:accessURL <https://www.legislation.gov.au/F2021L00334/2023-08-04/2023-08-04/text/original/epub/OEBPS/document_1/document_1.html#_Toc143507718> ;
    dcat:landingPage "https://www.legislation.gov.au/F2021L00334/2023-08-04/2023-08-04/text/original/epub/OEBPS/document_1/document_1.html#_Toc143507718"^^xsd:anyURI ;
    dcat:theme legcons:Part .

F2021L00334:74 a legcons:Part,
        owl:Class,
        dcat:Resource ;
    rdfs:label "Part - P74 Part 5 Variation of accreditation"@en-AU ;
    dct:hasPart F2021L00334:75,
        F2021L00334:76 ;
    dct:isPartOf F2021L00334:37 ;
    dct:isReferencedBy F2021L00334: ;
    rdfs:comment "Part 5 Variation of accreditation - Abrievated Graph Key: P74"@en-AU ;
    skos:broader F2021L00334:75,
        F2021L00334:76 ;
    skos:definition "Part 5 Variation of accreditation"@en-AU ;
    skos:narrower F2021L00334:37 ;
    skos:prefLabel "Part P74"@en-AU ;
    dcat:accessURL <https://www.legislation.gov.au/F2021L00334/2023-08-04/2023-08-04/text/original/epub/OEBPS/document_1/document_1.html#_Toc143507721> ;
    dcat:landingPage "https://www.legislation.gov.au/F2021L00334/2023-08-04/2023-08-04/text/original/epub/OEBPS/document_1/document_1.html#_Toc143507721"^^xsd:anyURI ;
    dcat:theme legcons:Part .

F2021L00334:79 a legcons:Part,
        owl:Class,
        dcat:Resource ;
    rdfs:label "Part - P79 Part 7 Obligations of managers of accredited properties etc"@en-AU ;
    dct:hasPart F2021L00334:80,
        F2021L00334:81 ;
    dct:isPartOf F2021L00334:37 ;
    dct:isReferencedBy F2021L00334: ;
    rdfs:comment "Part 7 Obligations of managers of accredited properties etc - Abrievated Graph Key: P79"@en-AU ;
    skos:broader F2021L00334:80,
        F2021L00334:81 ;
    skos:definition "Part 7 Obligations of managers of accredited properties etc"@en-AU ;
    skos:narrower F2021L00334:37 ;
    skos:prefLabel "Part P79"@en-AU ;
    dcat:accessURL <https://www.legislation.gov.au/F2021L00334/2023-08-04/2023-08-04/text/original/epub/OEBPS/document_1/document_1.html#_Toc143507726> ;
    dcat:landingPage "https://www.legislation.gov.au/F2021L00334/2023-08-04/2023-08-04/text/original/epub/OEBPS/document_1/document_1.html#_Toc143507726"^^xsd:anyURI ;
    dcat:theme legcons:Part .

F2021L00334:110 a legcons:Part,
        owl:Class,
        dcat:Resource ;
    rdfs:label "Part - P110 Part 5 Matters relating to applications"@en-AU ;
    dct:hasPart F2021L00334:111,
        F2021L00334:112,
        F2021L00334:113 ;
    dct:isPartOf F2021L00334:87 ;
    dct:isReferencedBy F2021L00334: ;
    rdfs:comment "Part 5 Matters relating to applications - Abrievated Graph Key: P110"@en-AU ;
    skos:broader F2021L00334:111,
        F2021L00334:112,
        F2021L00334:113 ;
    skos:definition "Part 5 Matters relating to applications"@en-AU ;
    skos:narrower F2021L00334:87 ;
    skos:prefLabel "Part P110"@en-AU ;
    dcat:accessURL <https://www.legislation.gov.au/F2021L00334/2023-08-04/2023-08-04/text/original/epub/OEBPS/document_1/document_1.html#_Toc143507757> ;
    dcat:landingPage "https://www.legislation.gov.au/F2021L00334/2023-08-04/2023-08-04/text/original/epub/OEBPS/document_1/document_1.html#_Toc143507757"^^xsd:anyURI ;
    dcat:theme legcons:Part .

F2021L00334:132 a legcons:Division,
        owl:Class,
        dcat:Resource ;
    rdfs:label "Division - D132 Division 1 Requirements for approval"@en-AU ;
    dct:hasPart F2021L00334:133,
        F2021L00334:134,
        F2021L00334:135 ;
    dct:isPartOf F2021L00334:131 ;
    dct:isReferencedBy F2021L00334: ;
    rdfs:comment "Division 1 Requirements for approval - Abrievated Graph Key: D132"@en-AU ;
    skos:broader F2021L00334:133,
        F2021L00334:134,
        F2021L00334:135 ;
    skos:definition "Division 1 Requirements for approval"@en-AU ;
    skos:narrower F2021L00334:131 ;
    skos:prefLabel "Division D132"@en-AU ;
    dcat:accessURL <https://www.legislation.gov.au/F2021L00334/2023-08-04/2023-08-04/text/original/epub/OEBPS/document_1/document_1.html#_Toc143507779> ;
    dcat:landingPage "https://www.legislation.gov.au/F2021L00334/2023-08-04/2023-08-04/text/original/epub/OEBPS/document_1/document_1.html#_Toc143507779"^^xsd:anyURI ;
    dcat:theme legcons:Division .

F2021L00334:203 a legcons:Division,
        owl:Class,
        dcat:Resource ;
    rdfs:label "Division - D203 Division 2 Conditions of approved arrangement"@en-AU ;
    dct:hasPart F2021L00334:204,
        F2021L00334:206,
        F2021L00334:208 ;
    dct:isPartOf F2021L00334:130 ;
    dct:isReferencedBy F2021L00334: ;
    rdfs:comment "Division 2 Conditions of approved arrangement - Abrievated Graph Key: D203"@en-AU ;
    skos:broader F2021L00334:204,
        F2021L00334:206,
        F2021L00334:208 ;
    skos:definition "Division 2 Conditions of approved arrangement"@en-AU ;
    skos:narrower F2021L00334:130 ;
    skos:prefLabel "Division D203"@en-AU ;
    dcat:accessURL <https://www.legislation.gov.au/F2021L00334/2023-08-04/2023-08-04/text/original/epub/OEBPS/document_1/document_1.html#_Toc143507850> ;
    dcat:landingPage "https://www.legislation.gov.au/F2021L00334/2023-08-04/2023-08-04/text/original/epub/OEBPS/document_1/document_1.html#_Toc143507850"^^xsd:anyURI ;
    dcat:theme legcons:Division .

F2021L00334:254 a legcons:Part,
        owl:Class,
        dcat:Resource ;
    rdfs:label "Part - P254 Part 2 Variation suspension and revocation of export permit"@en-AU ;
    dct:hasPart F2021L00334:255,
        F2021L00334:256,
        F2021L00334:257 ;
    dct:isPartOf F2021L00334:251 ;
    dct:isReferencedBy F2021L00334: ;
    rdfs:comment "Part 2 Variation suspension and revocation of export permit - Abrievated Graph Key: P254"@en-AU ;
    skos:broader F2021L00334:255,
        F2021L00334:256,
        F2021L00334:257 ;
    skos:definition "Part 2 Variation suspension and revocation of export permit"@en-AU ;
    skos:narrower F2021L00334:251 ;
    skos:prefLabel "Part P254"@en-AU ;
    dcat:accessURL <https://www.legislation.gov.au/F2021L00334/2023-08-04/2023-08-04/text/original/epub/OEBPS/document_1/document_1.html#_Toc143507901> ;
    dcat:landingPage "https://www.legislation.gov.au/F2021L00334/2023-08-04/2023-08-04/text/original/epub/OEBPS/document_1/document_1.html#_Toc143507901"^^xsd:anyURI ;
    dcat:theme legcons:Part .

F2021L00334:269 a legcons:Part,
        owl:Class,
        dcat:Resource ;
    rdfs:label "Part - P269 Part 2 Trade descriptions"@en-AU ;
    dct:hasPart F2021L00334:270,
        F2021L00334:271,
        F2021L00334:272 ;
    dct:isPartOf F2021L00334:263 ;
    dct:isReferencedBy F2021L00334: ;
    rdfs:comment "Part 2 Trade descriptions - Abrievated Graph Key: P269"@en-AU ;
    skos:broader F2021L00334:270,
        F2021L00334:271,
        F2021L00334:272 ;
    skos:definition "Part 2 Trade descriptions"@en-AU ;
    skos:narrower F2021L00334:263 ;
    skos:prefLabel "Part P269"@en-AU ;
    dcat:accessURL <https://www.legislation.gov.au/F2021L00334/2023-08-04/2023-08-04/text/original/epub/OEBPS/document_1/document_1.html#_Toc143507916> ;
    dcat:landingPage "https://www.legislation.gov.au/F2021L00334/2023-08-04/2023-08-04/text/original/epub/OEBPS/document_1/document_1.html#_Toc143507916"^^xsd:anyURI ;
    dcat:theme legcons:Part .

F2021L00334:302 a legcons:Division,
        owl:Class,
        dcat:Resource ;
    rdfs:label "Division - D302 Division 3 Marks resembling official marks"@en-AU ;
    dct:hasPart F2021L00334:303,
        F2021L00334:304,
        F2021L00334:305 ;
    dct:isPartOf F2021L00334:273 ;
    dct:isReferencedBy F2021L00334: ;
    rdfs:comment "Division 3 Marks resembling official marks - Abrievated Graph Key: D302"@en-AU ;
    skos:broader F2021L00334:303,
        F2021L00334:304,
        F2021L00334:305 ;
    skos:definition "Division 3 Marks resembling official marks"@en-AU ;
    skos:narrower F2021L00334:273 ;
    skos:prefLabel "Division D302"@en-AU ;
    dcat:accessURL <https://www.legislation.gov.au/F2021L00334/2023-08-04/2023-08-04/text/original/epub/OEBPS/document_1/document_1.html#_Toc143507949> ;
    dcat:landingPage "https://www.legislation.gov.au/F2021L00334/2023-08-04/2023-08-04/text/original/epub/OEBPS/document_1/document_1.html#_Toc143507949"^^xsd:anyURI ;
    dcat:theme legcons:Division .

F2021L00334:313 a legcons:Chapter,
        owl:Class,
        dcat:Resource ;
    rdfs:label "Chapter - C313 Chapter 9 Powers and officials"@en-AU ;
    dct:hasPart F2021L00334:314,
        F2021L00334:334,
        F2021L00334:336,
        F2021L00334:338 ;
    dct:isReferencedBy F2021L00334: ;
    rdfs:comment "Chapter 9 Powers and officials - Abrievated Graph Key: C313"@en-AU ;
    skos:broader F2021L00334:314,
        F2021L00334:334,
        F2021L00334:336,
        F2021L00334:338 ;
    skos:definition "Chapter 9 Powers and officials"@en-AU ;
    skos:prefLabel "Chapter C313"@en-AU ;
    dcat:accessURL <https://www.legislation.gov.au/F2021L00334/2023-08-04/2023-08-04/text/original/epub/OEBPS/document_1/document_1.html#_Toc143507960> ;
    dcat:landingPage "https://www.legislation.gov.au/F2021L00334/2023-08-04/2023-08-04/text/original/epub/OEBPS/document_1/document_1.html#_Toc143507960"^^xsd:anyURI ;
    dcat:theme legcons:Chapter .

F2021L00334:314 a legcons:Part,
        owl:Class,
        dcat:Resource ;
    rdfs:label "Part - P314 Part 1 Audits"@en-AU ;
    dct:hasPart F2021L00334:315,
        F2021L00334:317,
        F2021L00334:322 ;
    dct:isPartOf F2021L00334:313 ;
    dct:isReferencedBy F2021L00334: ;
    rdfs:comment "Part 1 Audits - Abrievated Graph Key: P314"@en-AU ;
    skos:broader F2021L00334:315,
        F2021L00334:317,
        F2021L00334:322 ;
    skos:definition "Part 1 Audits"@en-AU ;
    skos:narrower F2021L00334:313 ;
    skos:prefLabel "Part P314"@en-AU ;
    dcat:accessURL <https://www.legislation.gov.au/F2021L00334/2023-08-04/2023-08-04/text/original/epub/OEBPS/document_1/document_1.html#_Toc143507961> ;
    dcat:landingPage "https://www.legislation.gov.au/F2021L00334/2023-08-04/2023-08-04/text/original/epub/OEBPS/document_1/document_1.html#_Toc143507961"^^xsd:anyURI ;
    dcat:theme legcons:Part .

F2021L00334:408 a legcons:Part,
        owl:Class,
        dcat:Resource ;
    rdfs:label "Part - P408 Part 4 Other matters relating to export"@en-AU ;
    dct:hasPart F2021L00334:409,
        F2021L00334:411,
        F2021L00334:415 ;
    dct:isPartOf F2021L00334:385 ;
    dct:isReferencedBy F2021L00334: ;
    rdfs:comment "Part 4 Other matters relating to export - Abrievated Graph Key: P408"@en-AU ;
    skos:broader F2021L00334:409,
        F2021L00334:411,
        F2021L00334:415 ;
    skos:definition "Part 4 Other matters relating to export"@en-AU ;
    skos:narrower F2021L00334:385 ;
    skos:prefLabel "Part P408"@en-AU ;
    dcat:accessURL <https://www.legislation.gov.au/F2021L00334/2023-08-04/2023-08-04/text/original/epub/OEBPS/document_1/document_1.html#_Toc143508055> ;
    dcat:landingPage "https://www.legislation.gov.au/F2021L00334/2023-08-04/2023-08-04/text/original/epub/OEBPS/document_1/document_1.html#_Toc143508055"^^xsd:anyURI ;
    dcat:theme legcons:Part .

F2021L00334:411 a legcons:Division,
        owl:Class,
        dcat:Resource ;
    rdfs:label "Division - D411 Division 2 Official marks"@en-AU ;
    dct:hasPart F2021L00334:412,
        F2021L00334:413,
        F2021L00334:414 ;
    dct:isPartOf F2021L00334:408 ;
    dct:isReferencedBy F2021L00334: ;
    rdfs:comment "Division 2 Official marks - Abrievated Graph Key: D411"@en-AU ;
    skos:broader F2021L00334:412,
        F2021L00334:413,
        F2021L00334:414 ;
    skos:definition "Division 2 Official marks"@en-AU ;
    skos:narrower F2021L00334:408 ;
    skos:prefLabel "Division D411"@en-AU ;
    dcat:accessURL <https://www.legislation.gov.au/F2021L00334/2023-08-04/2023-08-04/text/original/epub/OEBPS/document_1/document_1.html#_Toc143508058> ;
    dcat:landingPage "https://www.legislation.gov.au/F2021L00334/2023-08-04/2023-08-04/text/original/epub/OEBPS/document_1/document_1.html#_Toc143508058"^^xsd:anyURI ;
    dcat:theme legcons:Division .

F2021L00334:419 a legcons:Division,
        owl:Class,
        dcat:Resource ;
    rdfs:label "Division - D419 Division 1 Approved auditors"@en-AU ;
    dct:hasPart F2021L00334:420,
        F2021L00334:421,
        F2021L00334:422 ;
    dct:isPartOf F2021L00334:418 ;
    dct:isReferencedBy F2021L00334: ;
    rdfs:comment "Division 1 Approved auditors - Abrievated Graph Key: D419"@en-AU ;
    skos:broader F2021L00334:420,
        F2021L00334:421,
        F2021L00334:422 ;
    skos:definition "Division 1 Approved auditors"@en-AU ;
    skos:narrower F2021L00334:418 ;
    skos:prefLabel "Division D419"@en-AU ;
    dcat:accessURL <https://www.legislation.gov.au/F2021L00334/2023-08-04/2023-08-04/text/original/epub/OEBPS/document_1/document_1.html#_Toc143508066> ;
    dcat:landingPage "https://www.legislation.gov.au/F2021L00334/2023-08-04/2023-08-04/text/original/epub/OEBPS/document_1/document_1.html#_Toc143508066"^^xsd:anyURI ;
    dcat:theme legcons:Division .

F2021L00334:423 a legcons:Division,
        owl:Class,
        dcat:Resource ;
    rdfs:label "Division - D423 Division 2 Decisions and dispositions"@en-AU ;
    dct:hasPart F2021L00334:424,
        F2021L00334:425,
        F2021L00334:426 ;
    dct:isPartOf F2021L00334:418 ;
    dct:isReferencedBy F2021L00334: ;
    rdfs:comment "Division 2 Decisions and dispositions - Abrievated Graph Key: D423"@en-AU ;
    skos:broader F2021L00334:424,
        F2021L00334:425,
        F2021L00334:426 ;
    skos:definition "Division 2 Decisions and dispositions"@en-AU ;
    skos:narrower F2021L00334:418 ;
    skos:prefLabel "Division D423"@en-AU ;
    dcat:accessURL <https://www.legislation.gov.au/F2021L00334/2023-08-04/2023-08-04/text/original/epub/OEBPS/document_1/document_1.html#_Toc143508070> ;
    dcat:landingPage "https://www.legislation.gov.au/F2021L00334/2023-08-04/2023-08-04/text/original/epub/OEBPS/document_1/document_1.html#_Toc143508070"^^xsd:anyURI ;
    dcat:theme legcons:Division .

F2021L00334:50 a legcons:Part,
        owl:Class,
        dcat:Resource ;
    rdfs:label "Part - P50 Part 3 Conditions of accreditation"@en-AU ;
    dct:hasPart F2021L00334:51,
        F2021L00334:58,
        F2021L00334:64 ;
    dct:isPartOf F2021L00334:37 ;
    dct:isReferencedBy F2021L00334: ;
    rdfs:comment "Part 3 Conditions of accreditation - Abrievated Graph Key: P50"@en-AU ;
    skos:broader F2021L00334:51,
        F2021L00334:58,
        F2021L00334:64 ;
    skos:definition "Part 3 Conditions of accreditation"@en-AU ;
    skos:narrower F2021L00334:37 ;
    skos:prefLabel "Part P50"@en-AU ;
    dcat:accessURL <https://www.legislation.gov.au/F2021L00334/2023-08-04/2023-08-04/text/original/epub/OEBPS/document_1/document_1.html#_Toc143507697> ;
    dcat:landingPage "https://www.legislation.gov.au/F2021L00334/2023-08-04/2023-08-04/text/original/epub/OEBPS/document_1/document_1.html#_Toc143507697"^^xsd:anyURI ;
    dcat:theme legcons:Part .

F2021L00334:246 a legcons:Part,
        owl:Class,
        dcat:Resource ;
    rdfs:label "Part - P246 Part 8 Matters relating to applications"@en-AU ;
    dct:hasPart F2021L00334:247,
        F2021L00334:248,
        F2021L00334:249,
        F2021L00334:250 ;
    dct:isPartOf F2021L00334:231 ;
    dct:isReferencedBy F2021L00334: ;
    rdfs:comment "Part 8 Matters relating to applications - Abrievated Graph Key: P246"@en-AU ;
    skos:broader F2021L00334:247,
        F2021L00334:248,
        F2021L00334:249,
        F2021L00334:250 ;
    skos:definition "Part 8 Matters relating to applications"@en-AU ;
    skos:narrower F2021L00334:231 ;
    skos:prefLabel "Part P246"@en-AU ;
    dcat:accessURL <https://www.legislation.gov.au/F2021L00334/2023-08-04/2023-08-04/text/original/epub/OEBPS/document_1/document_1.html#_Toc143507893> ;
    dcat:landingPage "https://www.legislation.gov.au/F2021L00334/2023-08-04/2023-08-04/text/original/epub/OEBPS/document_1/document_1.html#_Toc143507893"^^xsd:anyURI ;
    dcat:theme legcons:Part .

F2021L00334:258 a legcons:Part,
        owl:Class,
        dcat:Resource ;
    rdfs:label "Part - P258 Part 3 Other matters"@en-AU ;
    dct:hasPart F2021L00334:259,
        F2021L00334:260,
        F2021L00334:261,
        F2021L00334:262 ;
    dct:isPartOf F2021L00334:251 ;
    dct:isReferencedBy F2021L00334: ;
    rdfs:comment "Part 3 Other matters - Abrievated Graph Key: P258"@en-AU ;
    skos:broader F2021L00334:259,
        F2021L00334:260,
        F2021L00334:261,
        F2021L00334:262 ;
    skos:definition "Part 3 Other matters"@en-AU ;
    skos:narrower F2021L00334:251 ;
    skos:prefLabel "Part P258"@en-AU ;
    dcat:accessURL <https://www.legislation.gov.au/F2021L00334/2023-08-04/2023-08-04/text/original/epub/OEBPS/document_1/document_1.html#_Toc143507905> ;
    dcat:landingPage "https://www.legislation.gov.au/F2021L00334/2023-08-04/2023-08-04/text/original/epub/OEBPS/document_1/document_1.html#_Toc143507905"^^xsd:anyURI ;
    dcat:theme legcons:Part .

F2021L00334:264 a legcons:Part,
        owl:Class,
        dcat:Resource ;
    rdfs:label "Part - P264 Part 1 Notices of intention to export"@en-AU ;
    dct:hasPart F2021L00334:265,
        F2021L00334:266,
        F2021L00334:267,
        F2021L00334:268 ;
    dct:isPartOf F2021L00334:263 ;
    dct:isReferencedBy F2021L00334: ;
    rdfs:comment "Part 1 Notices of intention to export - Abrievated Graph Key: P264"@en-AU ;
    skos:broader F2021L00334:265,
        F2021L00334:266,
        F2021L00334:267,
        F2021L00334:268 ;
    skos:definition "Part 1 Notices of intention to export"@en-AU ;
    skos:narrower F2021L00334:263 ;
    skos:prefLabel "Part P264"@en-AU ;
    dcat:accessURL <https://www.legislation.gov.au/F2021L00334/2023-08-04/2023-08-04/text/original/epub/OEBPS/document_1/document_1.html#_Toc143507911> ;
    dcat:landingPage "https://www.legislation.gov.au/F2021L00334/2023-08-04/2023-08-04/text/original/epub/OEBPS/document_1/document_1.html#_Toc143507911"^^xsd:anyURI ;
    dcat:theme legcons:Part .

F2021L00334:273 a legcons:Part,
        owl:Class,
        dcat:Resource ;
    rdfs:label "Part - P273 Part 3 Official marks"@en-AU ;
    dct:hasPart F2021L00334:274,
        F2021L00334:289,
        F2021L00334:302,
        F2021L00334:306 ;
    dct:isPartOf F2021L00334:263 ;
    dct:isReferencedBy F2021L00334: ;
    rdfs:comment "Part 3 Official marks - Abrievated Graph Key: P273"@en-AU ;
    skos:broader F2021L00334:274,
        F2021L00334:289,
        F2021L00334:302,
        F2021L00334:306 ;
    skos:definition "Part 3 Official marks"@en-AU ;
    skos:narrower F2021L00334:263 ;
    skos:prefLabel "Part P273"@en-AU ;
    dcat:accessURL <https://www.legislation.gov.au/F2021L00334/2023-08-04/2023-08-04/text/original/epub/OEBPS/document_1/document_1.html#_Toc143507920> ;
    dcat:landingPage "https://www.legislation.gov.au/F2021L00334/2023-08-04/2023-08-04/text/original/epub/OEBPS/document_1/document_1.html#_Toc143507920"^^xsd:anyURI ;
    dcat:theme legcons:Part .

F2021L00334:317 a legcons:Division,
        owl:Class,
        dcat:Resource ;
    rdfs:label "Division - D317 Division 2 Conduct of audit etc"@en-AU ;
    dct:hasPart F2021L00334:318,
        F2021L00334:319,
        F2021L00334:320,
        F2021L00334:321 ;
    dct:isPartOf F2021L00334:314 ;
    dct:isReferencedBy F2021L00334: ;
    rdfs:comment "Division 2 Conduct of audit etc - Abrievated Graph Key: D317"@en-AU ;
    skos:broader F2021L00334:318,
        F2021L00334:319,
        F2021L00334:320,
        F2021L00334:321 ;
    skos:definition "Division 2 Conduct of audit etc"@en-AU ;
    skos:narrower F2021L00334:314 ;
    skos:prefLabel "Division D317"@en-AU ;
    dcat:accessURL <https://www.legislation.gov.au/F2021L00334/2023-08-04/2023-08-04/text/original/epub/OEBPS/document_1/document_1.html#_Toc143507964> ;
    dcat:landingPage "https://www.legislation.gov.au/F2021L00334/2023-08-04/2023-08-04/text/original/epub/OEBPS/document_1/document_1.html#_Toc143507964"^^xsd:anyURI ;
    dcat:theme legcons:Division .

F2021L00334:338 a legcons:Part,
        owl:Class,
        dcat:Resource ;
    rdfs:label "Part - P338 Part 4 Authorised officers"@en-AU ;
    dct:hasPart F2021L00334:339,
        F2021L00334:341,
        F2021L00334:356,
        F2021L00334:358 ;
    dct:isPartOf F2021L00334:313 ;
    dct:isReferencedBy F2021L00334: ;
    rdfs:comment "Part 4 Authorised officers - Abrievated Graph Key: P338"@en-AU ;
    skos:broader F2021L00334:339,
        F2021L00334:341,
        F2021L00334:356,
        F2021L00334:358 ;
    skos:definition "Part 4 Authorised officers"@en-AU ;
    skos:narrower F2021L00334:313 ;
    skos:prefLabel "Part P338"@en-AU ;
    dcat:accessURL <https://www.legislation.gov.au/F2021L00334/2023-08-04/2023-08-04/text/original/epub/OEBPS/document_1/document_1.html#_Toc143507985> ;
    dcat:landingPage "https://www.legislation.gov.au/F2021L00334/2023-08-04/2023-08-04/text/original/epub/OEBPS/document_1/document_1.html#_Toc143507985"^^xsd:anyURI ;
    dcat:theme legcons:Part .

F2021L00334:363 a legcons:Chapter,
        owl:Class,
        dcat:Resource ;
    rdfs:label "Chapter - C363 Chapter 11 Miscellaneous"@en-AU ;
    dct:hasPart F2021L00334:364,
        F2021L00334:366,
        F2021L00334:378,
        F2021L00334:380,
        F2021L00334:383 ;
    dct:isReferencedBy F2021L00334: ;
    rdfs:comment "Chapter 11 Miscellaneous - Abrievated Graph Key: C363"@en-AU ;
    skos:broader F2021L00334:364,
        F2021L00334:366,
        F2021L00334:378,
        F2021L00334:380,
        F2021L00334:383 ;
    skos:definition "Chapter 11 Miscellaneous"@en-AU ;
    skos:prefLabel "Chapter C363"@en-AU ;
    dcat:accessURL <https://www.legislation.gov.au/F2021L00334/2023-08-04/2023-08-04/text/original/epub/OEBPS/document_1/document_1.html#_Toc143508010> ;
    dcat:landingPage "https://www.legislation.gov.au/F2021L00334/2023-08-04/2023-08-04/text/original/epub/OEBPS/document_1/document_1.html#_Toc143508010"^^xsd:anyURI ;
    dcat:theme legcons:Chapter .

F2021L00334:42 a legcons:Division,
        owl:Class,
        dcat:Resource ;
    rdfs:label "Division - D42 Division 1 Requirements for accreditation"@en-AU ;
    dct:hasPart F2021L00334:43,
        F2021L00334:44,
        F2021L00334:45,
        F2021L00334:46 ;
    dct:isPartOf F2021L00334:41 ;
    dct:isReferencedBy F2021L00334: ;
    rdfs:comment "Division 1 Requirements for accreditation - Abrievated Graph Key: D42"@en-AU ;
    skos:broader F2021L00334:43,
        F2021L00334:44,
        F2021L00334:45,
        F2021L00334:46 ;
    skos:definition "Division 1 Requirements for accreditation"@en-AU ;
    skos:narrower F2021L00334:41 ;
    skos:prefLabel "Division D42"@en-AU ;
    dcat:accessURL <https://www.legislation.gov.au/F2021L00334/2023-08-04/2023-08-04/text/original/epub/OEBPS/document_1/document_1.html#_Toc143507689> ;
    dcat:landingPage "https://www.legislation.gov.au/F2021L00334/2023-08-04/2023-08-04/text/original/epub/OEBPS/document_1/document_1.html#_Toc143507689"^^xsd:anyURI ;
    dcat:theme legcons:Division .

F2021L00334:427 a legcons:Endnotes,
        owl:Class,
        dcat:Resource ;
    rdfs:label "Endnotes - E427 Endnotes"@en-AU ;
    dct:hasPart F2021L00334:428,
        F2021L00334:429,
        F2021L00334:430,
        F2021L00334:431 ;
    dct:isPartOf F2021L00334:385 ;
    dct:isReferencedBy F2021L00334: ;
    rdfs:comment "Endnotes - Abrievated Graph Key: E427"@en-AU ;
    skos:broader F2021L00334:428,
        F2021L00334:429,
        F2021L00334:430,
        F2021L00334:431 ;
    skos:definition "Endnotes"@en-AU ;
    skos:narrower F2021L00334:385 ;
    skos:prefLabel "Endnotes E427"@en-AU ;
    dcat:accessURL <https://www.legislation.gov.au/F2021L00334/2023-08-04/2023-08-04/text/original/epub/OEBPS/document_1/document_1.html#_Toc143508074> ;
    dcat:landingPage "https://www.legislation.gov.au/F2021L00334/2023-08-04/2023-08-04/text/original/epub/OEBPS/document_1/document_1.html#_Toc143508074"^^xsd:anyURI ;
    dcat:theme legcons:Endnotes .

F2021L00334:82 a legcons:Part,
        owl:Class,
        dcat:Resource ;
    rdfs:label "Part - P82 Part 8 Matters relating to applications"@en-AU ;
    dct:hasPart F2021L00334:83,
        F2021L00334:84,
        F2021L00334:85,
        F2021L00334:86 ;
    dct:isPartOf F2021L00334:37 ;
    dct:isReferencedBy F2021L00334: ;
    rdfs:comment "Part 8 Matters relating to applications - Abrievated Graph Key: P82"@en-AU ;
    skos:broader F2021L00334:83,
        F2021L00334:84,
        F2021L00334:85,
        F2021L00334:86 ;
    skos:definition "Part 8 Matters relating to applications"@en-AU ;
    skos:narrower F2021L00334:37 ;
    skos:prefLabel "Part P82"@en-AU ;
    dcat:accessURL <https://www.legislation.gov.au/F2021L00334/2023-08-04/2023-08-04/text/original/epub/OEBPS/document_1/document_1.html#_Toc143507729> ;
    dcat:landingPage "https://www.legislation.gov.au/F2021L00334/2023-08-04/2023-08-04/text/original/epub/OEBPS/document_1/document_1.html#_Toc143507729"^^xsd:anyURI ;
    dcat:theme legcons:Part .

F2021L00334:124 a legcons:Division,
        owl:Class,
        dcat:Resource ;
    rdfs:label "Division - D124 Division 2 Variation of meat inspection services"@en-AU ;
    dct:hasPart F2021L00334:125,
        F2021L00334:126,
        F2021L00334:127,
        F2021L00334:128,
        F2021L00334:129 ;
    dct:isPartOf F2021L00334:114 ;
    dct:isReferencedBy F2021L00334: ;
    rdfs:comment "Division 2 Variation of meat inspection services - Abrievated Graph Key: D124"@en-AU ;
    skos:broader F2021L00334:125,
        F2021L00334:126,
        F2021L00334:127,
        F2021L00334:128,
        F2021L00334:129 ;
    skos:definition "Division 2 Variation of meat inspection services"@en-AU ;
    skos:narrower F2021L00334:114 ;
    skos:prefLabel "Division D124"@en-AU ;
    dcat:accessURL <https://www.legislation.gov.au/F2021L00334/2023-08-04/2023-08-04/text/original/epub/OEBPS/document_1/document_1.html#_Toc143507771> ;
    dcat:landingPage "https://www.legislation.gov.au/F2021L00334/2023-08-04/2023-08-04/text/original/epub/OEBPS/document_1/document_1.html#_Toc143507771"^^xsd:anyURI ;
    dcat:theme legcons:Division .

F2021L00334:385 a legcons:Chapter,
        owl:Class,
        dcat:Resource ;
    rdfs:label "Chapter - C385 Chapter 12 Transitional provisions"@en-AU ;
    dct:hasPart F2021L00334:386,
        F2021L00334:388,
        F2021L00334:406,
        F2021L00334:408,
        F2021L00334:418,
        F2021L00334:427 ;
    dct:isReferencedBy F2021L00334: ;
    rdfs:comment "Chapter 12 Transitional provisions - Abrievated Graph Key: C385"@en-AU ;
    skos:broader F2021L00334:386,
        F2021L00334:388,
        F2021L00334:406,
        F2021L00334:408,
        F2021L00334:418,
        F2021L00334:427 ;
    skos:definition "Chapter 12 Transitional provisions"@en-AU ;
    skos:prefLabel "Chapter C385"@en-AU ;
    dcat:accessURL <https://www.legislation.gov.au/F2021L00334/2023-08-04/2023-08-04/text/original/epub/OEBPS/document_1/document_1.html#_Toc143508032> ;
    dcat:landingPage "https://www.legislation.gov.au/F2021L00334/2023-08-04/2023-08-04/text/original/epub/OEBPS/document_1/document_1.html#_Toc143508032"^^xsd:anyURI ;
    dcat:theme legcons:Chapter .

F2021L00334:58 a legcons:Division,
        owl:Class,
        dcat:Resource ;
    rdfs:label "Division - D58 Division 2 Conditions for accredited feedlots"@en-AU ;
    dct:hasPart F2021L00334:59,
        F2021L00334:60,
        F2021L00334:61,
        F2021L00334:62,
        F2021L00334:63 ;
    dct:isPartOf F2021L00334:50 ;
    dct:isReferencedBy F2021L00334: ;
    rdfs:comment "Division 2 Conditions for accredited feedlots - Abrievated Graph Key: D58"@en-AU ;
    skos:broader F2021L00334:59,
        F2021L00334:60,
        F2021L00334:61,
        F2021L00334:62,
        F2021L00334:63 ;
    skos:definition "Division 2 Conditions for accredited feedlots"@en-AU ;
    skos:narrower F2021L00334:50 ;
    skos:prefLabel "Division D58"@en-AU ;
    dcat:accessURL <https://www.legislation.gov.au/F2021L00334/2023-08-04/2023-08-04/text/original/epub/OEBPS/document_1/document_1.html#_Toc143507705> ;
    dcat:landingPage "https://www.legislation.gov.au/F2021L00334/2023-08-04/2023-08-04/text/original/epub/OEBPS/document_1/document_1.html#_Toc143507705"^^xsd:anyURI ;
    dcat:theme legcons:Division .

F2021L00334:87 a legcons:Chapter,
        owl:Class,
        dcat:Resource ;
    rdfs:label "Chapter - C87 Chapter 4 Registered establishments"@en-AU ;
    dct:hasPart F2021L00334:105,
        F2021L00334:108,
        F2021L00334:110,
        F2021L00334:114,
        F2021L00334:88,
        F2021L00334:98 ;
    dct:isReferencedBy F2021L00334: ;
    rdfs:comment "Chapter 4 Registered establishments - Abrievated Graph Key: C87"@en-AU ;
    skos:broader F2021L00334:105,
        F2021L00334:108,
        F2021L00334:110,
        F2021L00334:114,
        F2021L00334:88,
        F2021L00334:98 ;
    skos:definition "Chapter 4 Registered establishments"@en-AU ;
    skos:prefLabel "Chapter C87"@en-AU ;
    dcat:accessURL <https://www.legislation.gov.au/F2021L00334/2023-08-04/2023-08-04/text/original/epub/OEBPS/document_1/document_1.html#_Toc143507734> ;
    dcat:landingPage "https://www.legislation.gov.au/F2021L00334/2023-08-04/2023-08-04/text/original/epub/OEBPS/document_1/document_1.html#_Toc143507734"^^xsd:anyURI ;
    dcat:theme legcons:Chapter .

F2021L00334:208 a legcons:Subdivision,
        owl:Class,
        dcat:Resource ;
    rdfs:label "Subdivision - S208 Subdivision CManagement practices"@en-AU ;
    dct:hasPart F2021L00334:209,
        F2021L00334:210,
        F2021L00334:211,
        F2021L00334:212,
        F2021L00334:213,
        F2021L00334:214 ;
    dct:isPartOf F2021L00334:203 ;
    dct:isReferencedBy F2021L00334: ;
    rdfs:comment "Subdivision CManagement practices - Abrievated Graph Key: S208"@en-AU ;
    skos:broader F2021L00334:209,
        F2021L00334:210,
        F2021L00334:211,
        F2021L00334:212,
        F2021L00334:213,
        F2021L00334:214 ;
    skos:definition "Subdivision CManagement practices"@en-AU ;
    skos:narrower F2021L00334:203 ;
    skos:prefLabel "Subdivision S208"@en-AU ;
    dcat:accessURL <https://www.legislation.gov.au/F2021L00334/2023-08-04/2023-08-04/text/original/epub/OEBPS/document_1/document_1.html#_Toc143507855> ;
    dcat:landingPage "https://www.legislation.gov.au/F2021L00334/2023-08-04/2023-08-04/text/original/epub/OEBPS/document_1/document_1.html#_Toc143507855"^^xsd:anyURI ;
    dcat:theme legcons:Subdivision .

F2021L00334:22 a legcons:Part,
        owl:Class,
        dcat:Resource ;
    rdfs:label "Part - P22 Part 2 Exemptions"@en-AU ;
    dct:hasPart F2021L00334:23,
        F2021L00334:24,
        F2021L00334:25,
        F2021L00334:26,
        F2021L00334:27,
        F2021L00334:28 ;
    dct:isPartOf F2021L00334:14 ;
    dct:isReferencedBy F2021L00334: ;
    rdfs:comment "Part 2 Exemptions - Abrievated Graph Key: P22"@en-AU ;
    skos:broader F2021L00334:23,
        F2021L00334:24,
        F2021L00334:25,
        F2021L00334:26,
        F2021L00334:27,
        F2021L00334:28 ;
    skos:definition "Part 2 Exemptions"@en-AU ;
    skos:narrower F2021L00334:14 ;
    skos:prefLabel "Part P22"@en-AU ;
    dcat:accessURL <https://www.legislation.gov.au/F2021L00334/2023-08-04/2023-08-04/text/original/epub/OEBPS/document_1/document_1.html#_Toc143507669> ;
    dcat:landingPage "https://www.legislation.gov.au/F2021L00334/2023-08-04/2023-08-04/text/original/epub/OEBPS/document_1/document_1.html#_Toc143507669"^^xsd:anyURI ;
    dcat:theme legcons:Part .

F2021L00334:306 a legcons:Division,
        owl:Class,
        dcat:Resource ;
    rdfs:label "Division - D306 Division 4 Official marking devices"@en-AU ;
    dct:hasPart F2021L00334:307,
        F2021L00334:308,
        F2021L00334:309,
        F2021L00334:310,
        F2021L00334:311,
        F2021L00334:312 ;
    dct:isPartOf F2021L00334:273 ;
    dct:isReferencedBy F2021L00334: ;
    rdfs:comment "Division 4 Official marking devices - Abrievated Graph Key: D306"@en-AU ;
    skos:broader F2021L00334:307,
        F2021L00334:308,
        F2021L00334:309,
        F2021L00334:310,
        F2021L00334:311,
        F2021L00334:312 ;
    skos:definition "Division 4 Official marking devices"@en-AU ;
    skos:narrower F2021L00334:273 ;
    skos:prefLabel "Division D306"@en-AU ;
    dcat:accessURL <https://www.legislation.gov.au/F2021L00334/2023-08-04/2023-08-04/text/original/epub/OEBPS/document_1/document_1.html#_Toc143507953> ;
    dcat:landingPage "https://www.legislation.gov.au/F2021L00334/2023-08-04/2023-08-04/text/original/epub/OEBPS/document_1/document_1.html#_Toc143507953"^^xsd:anyURI ;
    dcat:theme legcons:Division .

F2021L00334:51 a legcons:Division,
        owl:Class,
        dcat:Resource ;
    rdfs:label "Division - D51 Division 1 Conditions for accredited farms"@en-AU ;
    dct:hasPart F2021L00334:52,
        F2021L00334:53,
        F2021L00334:54,
        F2021L00334:55,
        F2021L00334:56,
        F2021L00334:57 ;
    dct:isPartOf F2021L00334:50 ;
    dct:isReferencedBy F2021L00334: ;
    rdfs:comment "Division 1 Conditions for accredited farms - Abrievated Graph Key: D51"@en-AU ;
    skos:broader F2021L00334:52,
        F2021L00334:53,
        F2021L00334:54,
        F2021L00334:55,
        F2021L00334:56,
        F2021L00334:57 ;
    skos:definition "Division 1 Conditions for accredited farms"@en-AU ;
    skos:narrower F2021L00334:50 ;
    skos:prefLabel "Division D51"@en-AU ;
    dcat:accessURL <https://www.legislation.gov.au/F2021L00334/2023-08-04/2023-08-04/text/original/epub/OEBPS/document_1/document_1.html#_Toc143507698> ;
    dcat:landingPage "https://www.legislation.gov.au/F2021L00334/2023-08-04/2023-08-04/text/original/epub/OEBPS/document_1/document_1.html#_Toc143507698"^^xsd:anyURI ;
    dcat:theme legcons:Division .

F2021L00334:64 a legcons:Division,
        owl:Class,
        dcat:Resource ;
    rdfs:label "Division - D64 Division 3 Conditions for accredited saleyards"@en-AU ;
    dct:hasPart F2021L00334:65,
        F2021L00334:66,
        F2021L00334:67,
        F2021L00334:68,
        F2021L00334:69,
        F2021L00334:70 ;
    dct:isPartOf F2021L00334:50 ;
    dct:isReferencedBy F2021L00334: ;
    rdfs:comment "Division 3 Conditions for accredited saleyards - Abrievated Graph Key: D64"@en-AU ;
    skos:broader F2021L00334:65,
        F2021L00334:66,
        F2021L00334:67,
        F2021L00334:68,
        F2021L00334:69,
        F2021L00334:70 ;
    skos:definition "Division 3 Conditions for accredited saleyards"@en-AU ;
    skos:narrower F2021L00334:50 ;
    skos:prefLabel "Division D64"@en-AU ;
    dcat:accessURL <https://www.legislation.gov.au/F2021L00334/2023-08-04/2023-08-04/text/original/epub/OEBPS/document_1/document_1.html#_Toc143507711> ;
    dcat:landingPage "https://www.legislation.gov.au/F2021L00334/2023-08-04/2023-08-04/text/original/epub/OEBPS/document_1/document_1.html#_Toc143507711"^^xsd:anyURI ;
    dcat:theme legcons:Division .

F2021L00334:98 a legcons:Part,
        owl:Class,
        dcat:Resource ;
    rdfs:label "Part - P98 Part 2 Conditions of registration"@en-AU ;
    dct:hasPart F2021L00334:100,
        F2021L00334:101,
        F2021L00334:102,
        F2021L00334:103,
        F2021L00334:104,
        F2021L00334:99 ;
    dct:isPartOf F2021L00334:87 ;
    dct:isReferencedBy F2021L00334: ;
    rdfs:comment "Part 2 Conditions of registration - Abrievated Graph Key: P98"@en-AU ;
    skos:broader F2021L00334:100,
        F2021L00334:101,
        F2021L00334:102,
        F2021L00334:103,
        F2021L00334:104,
        F2021L00334:99 ;
    skos:definition "Part 2 Conditions of registration"@en-AU ;
    skos:narrower F2021L00334:87 ;
    skos:prefLabel "Part P98"@en-AU ;
    dcat:accessURL <https://www.legislation.gov.au/F2021L00334/2023-08-04/2023-08-04/text/original/epub/OEBPS/document_1/document_1.html#_Toc143507745> ;
    dcat:landingPage "https://www.legislation.gov.au/F2021L00334/2023-08-04/2023-08-04/text/original/epub/OEBPS/document_1/document_1.html#_Toc143507745"^^xsd:anyURI ;
    dcat:theme legcons:Part .

F2021L00334:131 a legcons:Part,
        owl:Class,
        dcat:Resource ;
    rdfs:label "Part - P131 Part 1 Approved arrangements for export operations other than Halal meat certification operations"@en-AU ;
    dct:hasPart F2021L00334:132,
        F2021L00334:136,
        F2021L00334:191,
        F2021L00334:192,
        F2021L00334:193,
        F2021L00334:194,
        F2021L00334:197 ;
    dct:isPartOf F2021L00334:130 ;
    dct:isReferencedBy F2021L00334: ;
    rdfs:comment "Part 1 Approved arrangements for export operations other than Halal meat certification operations - Abrievated Graph Key: P131"@en-AU ;
    skos:broader F2021L00334:132,
        F2021L00334:136,
        F2021L00334:191,
        F2021L00334:192,
        F2021L00334:193,
        F2021L00334:194,
        F2021L00334:197 ;
    skos:definition "Part 1 Approved arrangements for export operations other than Halal meat certification operations"@en-AU ;
    skos:narrower F2021L00334:130 ;
    skos:prefLabel "Part P131"@en-AU ;
    dcat:accessURL <https://www.legislation.gov.au/F2021L00334/2023-08-04/2023-08-04/text/original/epub/OEBPS/document_1/document_1.html#_Toc143507778> ;
    dcat:landingPage "https://www.legislation.gov.au/F2021L00334/2023-08-04/2023-08-04/text/original/epub/OEBPS/document_1/document_1.html#_Toc143507778"^^xsd:anyURI ;
    dcat:theme legcons:Part .

F2021L00334:231 a legcons:Chapter,
        owl:Class,
        dcat:Resource ;
    rdfs:label "Chapter - C231 Chapter 6 Meat export licences"@en-AU ;
    dct:hasPart F2021L00334:232,
        F2021L00334:234,
        F2021L00334:236,
        F2021L00334:238,
        F2021L00334:240,
        F2021L00334:242,
        F2021L00334:244,
        F2021L00334:246 ;
    dct:isReferencedBy F2021L00334: ;
    rdfs:comment "Chapter 6 Meat export licences - Abrievated Graph Key: C231"@en-AU ;
    skos:broader F2021L00334:232,
        F2021L00334:234,
        F2021L00334:236,
        F2021L00334:238,
        F2021L00334:240,
        F2021L00334:242,
        F2021L00334:244,
        F2021L00334:246 ;
    skos:definition "Chapter 6 Meat export licences"@en-AU ;
    skos:prefLabel "Chapter C231"@en-AU ;
    dcat:accessURL <https://www.legislation.gov.au/F2021L00334/2023-08-04/2023-08-04/text/original/epub/OEBPS/document_1/document_1.html#_Toc143507878> ;
    dcat:landingPage "https://www.legislation.gov.au/F2021L00334/2023-08-04/2023-08-04/text/original/epub/OEBPS/document_1/document_1.html#_Toc143507878"^^xsd:anyURI ;
    dcat:theme legcons:Chapter .

F2021L00334:29 a legcons:Part,
        owl:Class,
        dcat:Resource ;
    rdfs:label "Part - P29 Part 3 Government certificates"@en-AU ;
    dct:hasPart F2021L00334:30,
        F2021L00334:31,
        F2021L00334:32,
        F2021L00334:33,
        F2021L00334:34,
        F2021L00334:35,
        F2021L00334:36 ;
    dct:isPartOf F2021L00334:14 ;
    dct:isReferencedBy F2021L00334: ;
    rdfs:comment "Part 3 Government certificates - Abrievated Graph Key: P29"@en-AU ;
    skos:broader F2021L00334:30,
        F2021L00334:31,
        F2021L00334:32,
        F2021L00334:33,
        F2021L00334:34,
        F2021L00334:35,
        F2021L00334:36 ;
    skos:definition "Part 3 Government certificates"@en-AU ;
    skos:narrower F2021L00334:14 ;
    skos:prefLabel "Part P29"@en-AU ;
    dcat:accessURL <https://www.legislation.gov.au/F2021L00334/2023-08-04/2023-08-04/text/original/epub/OEBPS/document_1/document_1.html#_Toc143507676> ;
    dcat:landingPage "https://www.legislation.gov.au/F2021L00334/2023-08-04/2023-08-04/text/original/epub/OEBPS/document_1/document_1.html#_Toc143507676"^^xsd:anyURI ;
    dcat:theme legcons:Part .

F2021L00334:37 a legcons:Chapter,
        owl:Class,
        dcat:Resource ;
    rdfs:label "Chapter - C37 Chapter 3 Accredited properties"@en-AU ;
    dct:hasPart F2021L00334:38,
        F2021L00334:41,
        F2021L00334:50,
        F2021L00334:71,
        F2021L00334:74,
        F2021L00334:77,
        F2021L00334:79,
        F2021L00334:82 ;
    dct:isReferencedBy F2021L00334: ;
    rdfs:comment "Chapter 3 Accredited properties - Abrievated Graph Key: C37"@en-AU ;
    skos:broader F2021L00334:38,
        F2021L00334:41,
        F2021L00334:50,
        F2021L00334:71,
        F2021L00334:74,
        F2021L00334:77,
        F2021L00334:79,
        F2021L00334:82 ;
    skos:definition "Chapter 3 Accredited properties"@en-AU ;
    skos:prefLabel "Chapter C37"@en-AU ;
    dcat:accessURL <https://www.legislation.gov.au/F2021L00334/2023-08-04/2023-08-04/text/original/epub/OEBPS/document_1/document_1.html#_Toc143507684> ;
    dcat:landingPage "https://www.legislation.gov.au/F2021L00334/2023-08-04/2023-08-04/text/original/epub/OEBPS/document_1/document_1.html#_Toc143507684"^^xsd:anyURI ;
    dcat:theme legcons:Chapter .

F2021L00334:115 a legcons:Division,
        owl:Class,
        dcat:Resource ;
    rdfs:label "Division - D115 Division 1 Allocation of meat inspection services"@en-AU ;
    dct:hasPart F2021L00334:116,
        F2021L00334:117,
        F2021L00334:118,
        F2021L00334:119,
        F2021L00334:120,
        F2021L00334:121,
        F2021L00334:122,
        F2021L00334:123 ;
    dct:isPartOf F2021L00334:114 ;
    dct:isReferencedBy F2021L00334: ;
    rdfs:comment "Division 1 Allocation of meat inspection services - Abrievated Graph Key: D115"@en-AU ;
    skos:broader F2021L00334:116,
        F2021L00334:117,
        F2021L00334:118,
        F2021L00334:119,
        F2021L00334:120,
        F2021L00334:121,
        F2021L00334:122,
        F2021L00334:123 ;
    skos:definition "Division 1 Allocation of meat inspection services"@en-AU ;
    skos:narrower F2021L00334:114 ;
    skos:prefLabel "Division D115"@en-AU ;
    dcat:accessURL <https://www.legislation.gov.au/F2021L00334/2023-08-04/2023-08-04/text/original/epub/OEBPS/document_1/document_1.html#_Toc143507762> ;
    dcat:landingPage "https://www.legislation.gov.au/F2021L00334/2023-08-04/2023-08-04/text/original/epub/OEBPS/document_1/document_1.html#_Toc143507762"^^xsd:anyURI ;
    dcat:theme legcons:Division .

F2021L00334:88 a legcons:Part,
        owl:Class,
        dcat:Resource ;
    rdfs:label "Part - P88 Part 1 Requirements for registration"@en-AU ;
    dct:hasPart F2021L00334:89,
        F2021L00334:90,
        F2021L00334:91,
        F2021L00334:92,
        F2021L00334:93,
        F2021L00334:94,
        F2021L00334:95,
        F2021L00334:96,
        F2021L00334:97 ;
    dct:isPartOf F2021L00334:87 ;
    dct:isReferencedBy F2021L00334: ;
    rdfs:comment "Part 1 Requirements for registration - Abrievated Graph Key: P88"@en-AU ;
    skos:broader F2021L00334:89,
        F2021L00334:90,
        F2021L00334:91,
        F2021L00334:92,
        F2021L00334:93,
        F2021L00334:94,
        F2021L00334:95,
        F2021L00334:96,
        F2021L00334:97 ;
    skos:definition "Part 1 Requirements for registration"@en-AU ;
    skos:narrower F2021L00334:87 ;
    skos:prefLabel "Part P88"@en-AU ;
    dcat:accessURL <https://www.legislation.gov.au/F2021L00334/2023-08-04/2023-08-04/text/original/epub/OEBPS/document_1/document_1.html#_Toc143507735> ;
    dcat:landingPage "https://www.legislation.gov.au/F2021L00334/2023-08-04/2023-08-04/text/original/epub/OEBPS/document_1/document_1.html#_Toc143507735"^^xsd:anyURI ;
    dcat:theme legcons:Part .

F2021L00334:1 a legcons:Chapter,
        owl:Class,
        dcat:Resource ;
    rdfs:label "Chapter - C1 Chapter 1 Preliminary"@en-AU ;
    dct:hasPart F2021L00334:10,
        F2021L00334:11,
        F2021L00334:12,
        F2021L00334:13,
        F2021L00334:2,
        F2021L00334:3,
        F2021L00334:4,
        F2021L00334:5,
        F2021L00334:6,
        F2021L00334:7,
        F2021L00334:8,
        F2021L00334:9 ;
    dct:isReferencedBy F2021L00334: ;
    rdfs:comment "Chapter 1 Preliminary - Abrievated Graph Key: C1"@en-AU ;
    skos:broader F2021L00334:10,
        F2021L00334:11,
        F2021L00334:12,
        F2021L00334:13,
        F2021L00334:2,
        F2021L00334:3,
        F2021L00334:4,
        F2021L00334:5,
        F2021L00334:6,
        F2021L00334:7,
        F2021L00334:8,
        F2021L00334:9 ;
    skos:definition "Chapter 1 Preliminary"@en-AU ;
    skos:prefLabel "Chapter C1"@en-AU ;
    dcat:accessURL <https://www.legislation.gov.au/F2021L00334/2023-08-04/2023-08-04/text/original/epub/OEBPS/document_1/document_1.html#_Toc143507648> ;
    dcat:landingPage "https://www.legislation.gov.au/F2021L00334/2023-08-04/2023-08-04/text/original/epub/OEBPS/document_1/document_1.html#_Toc143507648"^^xsd:anyURI ;
    dcat:theme legcons:Chapter .

F2021L00334:322 a legcons:Division,
        owl:Class,
        dcat:Resource ;
    rdfs:label "Division - D322 Division 3 Approved auditors"@en-AU ;
    dct:hasPart F2021L00334:323,
        F2021L00334:324,
        F2021L00334:325,
        F2021L00334:326,
        F2021L00334:327,
        F2021L00334:328,
        F2021L00334:329,
        F2021L00334:330,
        F2021L00334:331,
        F2021L00334:332,
        F2021L00334:333 ;
    dct:isPartOf F2021L00334:314 ;
    dct:isReferencedBy F2021L00334: ;
    rdfs:comment "Division 3 Approved auditors - Abrievated Graph Key: D322"@en-AU ;
    skos:broader F2021L00334:323,
        F2021L00334:324,
        F2021L00334:325,
        F2021L00334:326,
        F2021L00334:327,
        F2021L00334:328,
        F2021L00334:329,
        F2021L00334:330,
        F2021L00334:331,
        F2021L00334:332,
        F2021L00334:333 ;
    skos:definition "Division 3 Approved auditors"@en-AU ;
    skos:narrower F2021L00334:314 ;
    skos:prefLabel "Division D322"@en-AU ;
    dcat:accessURL <https://www.legislation.gov.au/F2021L00334/2023-08-04/2023-08-04/text/original/epub/OEBPS/document_1/document_1.html#_Toc143507969> ;
    dcat:landingPage "https://www.legislation.gov.au/F2021L00334/2023-08-04/2023-08-04/text/original/epub/OEBPS/document_1/document_1.html#_Toc143507969"^^xsd:anyURI ;
    dcat:theme legcons:Division .

F2021L00334:366 a legcons:Part,
        owl:Class,
        dcat:Resource ;
    rdfs:label "Part - P366 Part 2 Records"@en-AU ;
    dct:hasPart F2021L00334:367,
        F2021L00334:368,
        F2021L00334:369,
        F2021L00334:370,
        F2021L00334:371,
        F2021L00334:372,
        F2021L00334:373,
        F2021L00334:374,
        F2021L00334:375,
        F2021L00334:376,
        F2021L00334:377 ;
    dct:isPartOf F2021L00334:363 ;
    dct:isReferencedBy F2021L00334: ;
    rdfs:comment "Part 2 Records - Abrievated Graph Key: P366"@en-AU ;
    skos:broader F2021L00334:367,
        F2021L00334:368,
        F2021L00334:369,
        F2021L00334:370,
        F2021L00334:371,
        F2021L00334:372,
        F2021L00334:373,
        F2021L00334:374,
        F2021L00334:375,
        F2021L00334:376,
        F2021L00334:377 ;
    skos:definition "Part 2 Records"@en-AU ;
    skos:narrower F2021L00334:363 ;
    skos:prefLabel "Part P366"@en-AU ;
    dcat:accessURL <https://www.legislation.gov.au/F2021L00334/2023-08-04/2023-08-04/text/original/epub/OEBPS/document_1/document_1.html#_Toc143508013> ;
    dcat:landingPage "https://www.legislation.gov.au/F2021L00334/2023-08-04/2023-08-04/text/original/epub/OEBPS/document_1/document_1.html#_Toc143508013"^^xsd:anyURI ;
    dcat:theme legcons:Part .

F2021L00334:130 a legcons:Chapter,
        owl:Class,
        dcat:Resource ;
    rdfs:label "Chapter - C130 Chapter 5 Approved arrangements"@en-AU ;
    dct:hasPart F2021L00334:131,
        F2021L00334:199,
        F2021L00334:200,
        F2021L00334:203,
        F2021L00334:215,
        F2021L00334:217,
        F2021L00334:222,
        F2021L00334:224,
        F2021L00334:226,
        F2021L00334:227,
        F2021L00334:228,
        F2021L00334:229,
        F2021L00334:230 ;
    dct:isReferencedBy F2021L00334: ;
    rdfs:comment "Chapter 5 Approved arrangements - Abrievated Graph Key: C130"@en-AU ;
    skos:broader F2021L00334:131,
        F2021L00334:199,
        F2021L00334:200,
        F2021L00334:203,
        F2021L00334:215,
        F2021L00334:217,
        F2021L00334:222,
        F2021L00334:224,
        F2021L00334:226,
        F2021L00334:227,
        F2021L00334:228,
        F2021L00334:229,
        F2021L00334:230 ;
    skos:definition "Chapter 5 Approved arrangements"@en-AU ;
    skos:prefLabel "Chapter C130"@en-AU ;
    dcat:accessURL <https://www.legislation.gov.au/F2021L00334/2023-08-04/2023-08-04/text/original/epub/OEBPS/document_1/document_1.html#_Toc143507777> ;
    dcat:landingPage "https://www.legislation.gov.au/F2021L00334/2023-08-04/2023-08-04/text/original/epub/OEBPS/document_1/document_1.html#_Toc143507777"^^xsd:anyURI ;
    dcat:theme legcons:Chapter .

F2021L00334:289 a legcons:Division,
        owl:Class,
        dcat:Resource ;
    rdfs:label "Division - D289 Division 2 General rules relating to official marks"@en-AU ;
    dct:hasPart F2021L00334:290,
        F2021L00334:291,
        F2021L00334:292,
        F2021L00334:293,
        F2021L00334:294,
        F2021L00334:295,
        F2021L00334:296,
        F2021L00334:297,
        F2021L00334:298,
        F2021L00334:299,
        F2021L00334:300,
        F2021L00334:301 ;
    dct:isPartOf F2021L00334:273 ;
    dct:isReferencedBy F2021L00334: ;
    rdfs:comment "Division 2 General rules relating to official marks - Abrievated Graph Key: D289"@en-AU ;
    skos:broader F2021L00334:290,
        F2021L00334:291,
        F2021L00334:292,
        F2021L00334:293,
        F2021L00334:294,
        F2021L00334:295,
        F2021L00334:296,
        F2021L00334:297,
        F2021L00334:298,
        F2021L00334:299,
        F2021L00334:300,
        F2021L00334:301 ;
    skos:definition "Division 2 General rules relating to official marks"@en-AU ;
    skos:narrower F2021L00334:273 ;
    skos:prefLabel "Division D289"@en-AU ;
    dcat:accessURL <https://www.legislation.gov.au/F2021L00334/2023-08-04/2023-08-04/text/original/epub/OEBPS/document_1/document_1.html#_Toc143507936> ;
    dcat:landingPage "https://www.legislation.gov.au/F2021L00334/2023-08-04/2023-08-04/text/original/epub/OEBPS/document_1/document_1.html#_Toc143507936"^^xsd:anyURI ;
    dcat:theme legcons:Division .

F2021L00334:274 a legcons:Division,
        owl:Class,
        dcat:Resource ;
    rdfs:label "Division - D274 Division 1 Marks that are official marks"@en-AU ;
    dct:hasPart F2021L00334:275,
        F2021L00334:276,
        F2021L00334:277,
        F2021L00334:278,
        F2021L00334:279,
        F2021L00334:280,
        F2021L00334:281,
        F2021L00334:282,
        F2021L00334:283,
        F2021L00334:284,
        F2021L00334:285,
        F2021L00334:286,
        F2021L00334:287,
        F2021L00334:288 ;
    dct:isPartOf F2021L00334:273 ;
    dct:isReferencedBy F2021L00334: ;
    rdfs:comment "Division 1 Marks that are official marks - Abrievated Graph Key: D274"@en-AU ;
    skos:broader F2021L00334:275,
        F2021L00334:276,
        F2021L00334:277,
        F2021L00334:278,
        F2021L00334:279,
        F2021L00334:280,
        F2021L00334:281,
        F2021L00334:282,
        F2021L00334:283,
        F2021L00334:284,
        F2021L00334:285,
        F2021L00334:286,
        F2021L00334:287,
        F2021L00334:288 ;
    skos:definition "Division 1 Marks that are official marks"@en-AU ;
    skos:narrower F2021L00334:273 ;
    skos:prefLabel "Division D274"@en-AU ;
    dcat:accessURL <https://www.legislation.gov.au/F2021L00334/2023-08-04/2023-08-04/text/original/epub/OEBPS/document_1/document_1.html#_Toc143507921> ;
    dcat:landingPage "https://www.legislation.gov.au/F2021L00334/2023-08-04/2023-08-04/text/original/epub/OEBPS/document_1/document_1.html#_Toc143507921"^^xsd:anyURI ;
    dcat:theme legcons:Division .

F2021L00334:341 a legcons:Division,
        owl:Class,
        dcat:Resource ;
    rdfs:label "Division - D341 Division 2 Functions and powers"@en-AU ;
    dct:hasPart F2021L00334:342,
        F2021L00334:343,
        F2021L00334:344,
        F2021L00334:345,
        F2021L00334:346,
        F2021L00334:347,
        F2021L00334:348,
        F2021L00334:349,
        F2021L00334:350,
        F2021L00334:351,
        F2021L00334:352,
        F2021L00334:353,
        F2021L00334:354,
        F2021L00334:355 ;
    dct:isPartOf F2021L00334:338 ;
    dct:isReferencedBy F2021L00334: ;
    rdfs:comment "Division 2 Functions and powers - Abrievated Graph Key: D341"@en-AU ;
    skos:broader F2021L00334:342,
        F2021L00334:343,
        F2021L00334:344,
        F2021L00334:345,
        F2021L00334:346,
        F2021L00334:347,
        F2021L00334:348,
        F2021L00334:349,
        F2021L00334:350,
        F2021L00334:351,
        F2021L00334:352,
        F2021L00334:353,
        F2021L00334:354,
        F2021L00334:355 ;
    skos:definition "Division 2 Functions and powers"@en-AU ;
    skos:narrower F2021L00334:338 ;
    skos:prefLabel "Division D341"@en-AU ;
    dcat:accessURL <https://www.legislation.gov.au/F2021L00334/2023-08-04/2023-08-04/text/original/epub/OEBPS/document_1/document_1.html#_Toc143507988> ;
    dcat:landingPage "https://www.legislation.gov.au/F2021L00334/2023-08-04/2023-08-04/text/original/epub/OEBPS/document_1/document_1.html#_Toc143507988"^^xsd:anyURI ;
    dcat:theme legcons:Division .

F2021L00334:388 a legcons:Part,
        owl:Class,
        dcat:Resource ;
    rdfs:label "Part - P388 Part 2 Registered establishments meat inspection services"@en-AU ;
    dct:hasPart F2021L00334:389,
        F2021L00334:390,
        F2021L00334:391,
        F2021L00334:392,
        F2021L00334:393,
        F2021L00334:394,
        F2021L00334:395,
        F2021L00334:396,
        F2021L00334:397,
        F2021L00334:398,
        F2021L00334:399,
        F2021L00334:400,
        F2021L00334:401,
        F2021L00334:402,
        F2021L00334:403,
        F2021L00334:404,
        F2021L00334:405 ;
    dct:isPartOf F2021L00334:385 ;
    dct:isReferencedBy F2021L00334: ;
    rdfs:comment "Part 2 Registered establishments meat inspection services - Abrievated Graph Key: P388"@en-AU ;
    skos:broader F2021L00334:389,
        F2021L00334:390,
        F2021L00334:391,
        F2021L00334:392,
        F2021L00334:393,
        F2021L00334:394,
        F2021L00334:395,
        F2021L00334:396,
        F2021L00334:397,
        F2021L00334:398,
        F2021L00334:399,
        F2021L00334:400,
        F2021L00334:401,
        F2021L00334:402,
        F2021L00334:403,
        F2021L00334:404,
        F2021L00334:405 ;
    skos:definition "Part 2 Registered establishments meat inspection services"@en-AU ;
    skos:narrower F2021L00334:385 ;
    skos:prefLabel "Part P388"@en-AU ;
    dcat:accessURL <https://www.legislation.gov.au/F2021L00334/2023-08-04/2023-08-04/text/original/epub/OEBPS/document_1/document_1.html#_Toc143508035> ;
    dcat:landingPage "https://www.legislation.gov.au/F2021L00334/2023-08-04/2023-08-04/text/original/epub/OEBPS/document_1/document_1.html#_Toc143508035"^^xsd:anyURI ;
    dcat:theme legcons:Part .

F2021L00334:136 a legcons:Division,
        owl:Class,
        dcat:Resource ;
    rdfs:label "Division - D136 Division 2 Conditions of approved arrangement"@en-AU ;
    dct:hasPart F2021L00334:137,
        F2021L00334:139,
        F2021L00334:140,
        F2021L00334:141,
        F2021L00334:142,
        F2021L00334:143,
        F2021L00334:144,
        F2021L00334:145,
        F2021L00334:146,
        F2021L00334:147,
        F2021L00334:148,
        F2021L00334:149,
        F2021L00334:150,
        F2021L00334:151,
        F2021L00334:152,
        F2021L00334:153,
        F2021L00334:154,
        F2021L00334:155,
        F2021L00334:156,
        F2021L00334:157,
        F2021L00334:158,
        F2021L00334:159,
        F2021L00334:160,
        F2021L00334:161,
        F2021L00334:162,
        F2021L00334:163,
        F2021L00334:164,
        F2021L00334:165,
        F2021L00334:166,
        F2021L00334:167,
        F2021L00334:168,
        F2021L00334:169,
        F2021L00334:170,
        F2021L00334:171,
        F2021L00334:172,
        F2021L00334:173,
        F2021L00334:174,
        F2021L00334:175,
        F2021L00334:176,
        F2021L00334:177,
        F2021L00334:178,
        F2021L00334:179,
        F2021L00334:180,
        F2021L00334:181,
        F2021L00334:182,
        F2021L00334:183,
        F2021L00334:184,
        F2021L00334:185,
        F2021L00334:186,
        F2021L00334:187,
        F2021L00334:188,
        F2021L00334:189,
        F2021L00334:190 ;
    dct:isPartOf F2021L00334:131 ;
    dct:isReferencedBy F2021L00334: ;
    rdfs:comment "Division 2 Conditions of approved arrangement - Abrievated Graph Key: D136"@en-AU ;
    skos:broader F2021L00334:137,
        F2021L00334:139,
        F2021L00334:140,
        F2021L00334:141,
        F2021L00334:142,
        F2021L00334:143,
        F2021L00334:144,
        F2021L00334:145,
        F2021L00334:146,
        F2021L00334:147,
        F2021L00334:148,
        F2021L00334:149,
        F2021L00334:150,
        F2021L00334:151,
        F2021L00334:152,
        F2021L00334:153,
        F2021L00334:154,
        F2021L00334:155,
        F2021L00334:156,
        F2021L00334:157,
        F2021L00334:158,
        F2021L00334:159,
        F2021L00334:160,
        F2021L00334:161,
        F2021L00334:162,
        F2021L00334:163,
        F2021L00334:164,
        F2021L00334:165,
        F2021L00334:166,
        F2021L00334:167,
        F2021L00334:168,
        F2021L00334:169,
        F2021L00334:170,
        F2021L00334:171,
        F2021L00334:172,
        F2021L00334:173,
        F2021L00334:174,
        F2021L00334:175,
        F2021L00334:176,
        F2021L00334:177,
        F2021L00334:178,
        F2021L00334:179,
        F2021L00334:180,
        F2021L00334:181,
        F2021L00334:182,
        F2021L00334:183,
        F2021L00334:184,
        F2021L00334:185,
        F2021L00334:186,
        F2021L00334:187,
        F2021L00334:188,
        F2021L00334:189,
        F2021L00334:190 ;
    skos:definition "Division 2 Conditions of approved arrangement"@en-AU ;
    skos:narrower F2021L00334:131 ;
    skos:prefLabel "Division D136"@en-AU ;
    dcat:accessURL <https://www.legislation.gov.au/F2021L00334/2023-08-04/2023-08-04/text/original/epub/OEBPS/document_1/document_1.html#_Toc143507783> ;
    dcat:landingPage "https://www.legislation.gov.au/F2021L00334/2023-08-04/2023-08-04/text/original/epub/OEBPS/document_1/document_1.html#_Toc143507783"^^xsd:anyURI ;
    dcat:theme legcons:Division .

F2021L00334: a owl:Class,
        dcat:Dataset,
        dcat:Resource ;
    rdfs:label "Export Control (Meat and Meat Products) Rules 2021" ;
    dct:Jurisdiction " Department of Agriculture, Fisheries and Forestry "@en-AU ;
    dct:created "2024-08-30T15:13:01.693621"^^xsd:dateTime ;
    dct:creator "https://orcid.org/0009-0007-8434-7325"^^xsd:anyURI ;
    dct:date "2023-08-04T00:00:00+10:00"^^xsd:dateTime ;
    dct:description "Export Control (Meat and Meat Products) Rules 2021"@en-AU ;
    dct:identifier "https://www.legislation.gov.au/F2021L00334/latest"^^xsd:anyURI ;
    dct:license <https://creativecommons.org/licenses/by-sa/4.0/> ;
    dct:source "scheme=AGLSTERMS.AglsAgent; corporateName=Office Parliamentary Counsel; address=Locked Bag 30 Kingston ACT 2604; contact=+61 2 6120 1400"@en-AU ;
    dct:subject "Export Control (Meat and Meat Products) Rules 2021"@en-AU ;
    dct:title "Export Control (Meat and Meat Products) Rules 2021"@en-AU ;
    owl:imports legcons: ;
    dcat:theme legcons:Chapter,
        legcons:Division,
        legcons:Endnotes,
        legcons:Item,
        legcons:Part,
        legcons:Subdivision ;
    schema:identifier "F2021L00334" ;
    schema:status "In force" ;
    schema:version "F2023C00739 (C03)" .

