@prefix F2021L00304: <http://example.org/au/leg/dataset/F2021L00304/> .
@prefix dcat: <http://www.w3.org/ns/dcat#> .
@prefix dct: <http://purl.org/dc/terms/> .
@prefix legcons: <http://example.org/au/leg/concepts/> .
@prefix owl: <http://www.w3.org/2002/07/owl#> .
@prefix rdfs: <http://www.w3.org/2000/01/rdf-schema#> .
@prefix schema: <https://schema.org/> .
@prefix skos: <http://www.w3.org/2004/02/skos/core#> .
@prefix xsd: <http://www.w3.org/2001/XMLSchema#> .

F2021L00304:100 a legcons:Item,
        owl:Class,
        dcat:Resource ;
    rdfs:label "Item - I100 5 30  Trade descriptions applied to packaging etc"@en-AU ;
    dct:isPartOf F2021L00304:96 ;
    dct:isReferencedBy F2021L00304: ;
    rdfs:comment "5 30  Trade descriptions applied to packaging etc - Abrievated Graph Key: I100"@en-AU ;
    skos:definition "5 30  Trade descriptions applied to packaging etc"@en-AU ;
    skos:narrower F2021L00304:96 ;
    skos:prefLabel "Item I100"@en-AU ;
    dcat:accessURL <https://www.legislation.gov.au/F2021L00304/asmade/2021-03-24/text/original/epub/OEBPS/document_1/document_1.html#_Toc65844106> ;
    dcat:landingPage "https://www.legislation.gov.au/F2021L00304/asmade/2021-03-24/text/original/epub/OEBPS/document_1/document_1.html#_Toc65844106"^^xsd:anyURI ;
    dcat:theme legcons:Item .

F2021L00304:102 a legcons:Item,
        owl:Class,
        dcat:Resource ;
    rdfs:label "Item - I102 5 31  Alteration of or interference with official mark"@en-AU ;
    dct:isPartOf F2021L00304:101 ;
    dct:isReferencedBy F2021L00304: ;
    rdfs:comment "5 31  Alteration of or interference with official mark - Abrievated Graph Key: I102"@en-AU ;
    skos:definition "5 31  Alteration of or interference with official mark"@en-AU ;
    skos:narrower F2021L00304:101 ;
    skos:prefLabel "Item I102"@en-AU ;
    dcat:accessURL <https://www.legislation.gov.au/F2021L00304/asmade/2021-03-24/text/original/epub/OEBPS/document_1/document_1.html#_Toc65844108> ;
    dcat:landingPage "https://www.legislation.gov.au/F2021L00304/asmade/2021-03-24/text/original/epub/OEBPS/document_1/document_1.html#_Toc65844108"^^xsd:anyURI ;
    dcat:theme legcons:Item .

F2021L00304:104 a legcons:Item,
        owl:Class,
        dcat:Resource ;
    rdfs:label "Item - I104 5 32  Segregation identification and traceabilitygeneral"@en-AU ;
    dct:isPartOf F2021L00304:103 ;
    dct:isReferencedBy F2021L00304: ;
    rdfs:comment "5 32  Segregation identification and traceabilitygeneral - Abrievated Graph Key: I104"@en-AU ;
    skos:definition "5 32  Segregation identification and traceabilitygeneral"@en-AU ;
    skos:narrower F2021L00304:103 ;
    skos:prefLabel "Item I104"@en-AU ;
    dcat:accessURL <https://www.legislation.gov.au/F2021L00304/asmade/2021-03-24/text/original/epub/OEBPS/document_1/document_1.html#_Toc65844110> ;
    dcat:landingPage "https://www.legislation.gov.au/F2021L00304/asmade/2021-03-24/text/original/epub/OEBPS/document_1/document_1.html#_Toc65844110"^^xsd:anyURI ;
    dcat:theme legcons:Item .

F2021L00304:105 a legcons:Item,
        owl:Class,
        dcat:Resource ;
    rdfs:label "Item - I105 5 33  Establishments where milk or milk products that are not for export etc are prepared"@en-AU ;
    dct:isPartOf F2021L00304:103 ;
    dct:isReferencedBy F2021L00304: ;
    rdfs:comment "5 33  Establishments where milk or milk products that are not for export etc are prepared - Abrievated Graph Key: I105"@en-AU ;
    skos:definition "5 33  Establishments where milk or milk products that are not for export etc are prepared"@en-AU ;
    skos:narrower F2021L00304:103 ;
    skos:prefLabel "Item I105"@en-AU ;
    dcat:accessURL <https://www.legislation.gov.au/F2021L00304/asmade/2021-03-24/text/original/epub/OEBPS/document_1/document_1.html#_Toc65844111> ;
    dcat:landingPage "https://www.legislation.gov.au/F2021L00304/asmade/2021-03-24/text/original/epub/OEBPS/document_1/document_1.html#_Toc65844111"^^xsd:anyURI ;
    dcat:theme legcons:Item .

F2021L00304:106 a legcons:Item,
        owl:Class,
        dcat:Resource ;
    rdfs:label "Item - I106 5 34  Integritygeneral"@en-AU ;
    dct:isPartOf F2021L00304:103 ;
    dct:isReferencedBy F2021L00304: ;
    rdfs:comment "5 34  Integritygeneral - Abrievated Graph Key: I106"@en-AU ;
    skos:definition "5 34  Integritygeneral"@en-AU ;
    skos:narrower F2021L00304:103 ;
    skos:prefLabel "Item I106"@en-AU ;
    dcat:accessURL <https://www.legislation.gov.au/F2021L00304/asmade/2021-03-24/text/original/epub/OEBPS/document_1/document_1.html#_Toc65844112> ;
    dcat:landingPage "https://www.legislation.gov.au/F2021L00304/asmade/2021-03-24/text/original/epub/OEBPS/document_1/document_1.html#_Toc65844112"^^xsd:anyURI ;
    dcat:theme legcons:Item .

F2021L00304:108 a legcons:Item,
        owl:Class,
        dcat:Resource ;
    rdfs:label "Item - I108 5 35  Information and declarations relating to transferred prescribed milk or milk products"@en-AU ;
    dct:isPartOf F2021L00304:107 ;
    dct:isReferencedBy F2021L00304: ;
    rdfs:comment "5 35  Information and declarations relating to transferred prescribed milk or milk products - Abrievated Graph Key: I108"@en-AU ;
    skos:definition "5 35  Information and declarations relating to transferred prescribed milk or milk products"@en-AU ;
    skos:narrower F2021L00304:107 ;
    skos:prefLabel "Item I108"@en-AU ;
    dcat:accessURL <https://www.legislation.gov.au/F2021L00304/asmade/2021-03-24/text/original/epub/OEBPS/document_1/document_1.html#_Toc65844114> ;
    dcat:landingPage "https://www.legislation.gov.au/F2021L00304/asmade/2021-03-24/text/original/epub/OEBPS/document_1/document_1.html#_Toc65844114"^^xsd:anyURI ;
    dcat:theme legcons:Item .

F2021L00304:109 a legcons:Item,
        owl:Class,
        dcat:Resource ;
    rdfs:label "Item - I109 5 36  Information and declarations not received or inaccurate or incomplete"@en-AU ;
    dct:isPartOf F2021L00304:107 ;
    dct:isReferencedBy F2021L00304: ;
    rdfs:comment "5 36  Information and declarations not received or inaccurate or incomplete - Abrievated Graph Key: I109"@en-AU ;
    skos:definition "5 36  Information and declarations not received or inaccurate or incomplete"@en-AU ;
    skos:narrower F2021L00304:107 ;
    skos:prefLabel "Item I109"@en-AU ;
    dcat:accessURL <https://www.legislation.gov.au/F2021L00304/asmade/2021-03-24/text/original/epub/OEBPS/document_1/document_1.html#_Toc65844115> ;
    dcat:landingPage "https://www.legislation.gov.au/F2021L00304/asmade/2021-03-24/text/original/epub/OEBPS/document_1/document_1.html#_Toc65844115"^^xsd:anyURI ;
    dcat:theme legcons:Item .

F2021L00304:111 a legcons:Item,
        owl:Class,
        dcat:Resource ;
    rdfs:label "Item - I111 5 37  Management practices organisational structure resources and personnel"@en-AU ;
    dct:isPartOf F2021L00304:110 ;
    dct:isReferencedBy F2021L00304: ;
    rdfs:comment "5 37  Management practices organisational structure resources and personnel - Abrievated Graph Key: I111"@en-AU ;
    skos:definition "5 37  Management practices organisational structure resources and personnel"@en-AU ;
    skos:narrower F2021L00304:110 ;
    skos:prefLabel "Item I111"@en-AU ;
    dcat:accessURL <https://www.legislation.gov.au/F2021L00304/asmade/2021-03-24/text/original/epub/OEBPS/document_1/document_1.html#_Toc65844117> ;
    dcat:landingPage "https://www.legislation.gov.au/F2021L00304/asmade/2021-03-24/text/original/epub/OEBPS/document_1/document_1.html#_Toc65844117"^^xsd:anyURI ;
    dcat:theme legcons:Item .

F2021L00304:112 a legcons:Item,
        owl:Class,
        dcat:Resource ;
    rdfs:label "Item - I112 5 38  Verification of compliance with the Act and other matters"@en-AU ;
    dct:isPartOf F2021L00304:110 ;
    dct:isReferencedBy F2021L00304: ;
    rdfs:comment "5 38  Verification of compliance with the Act and other matters - Abrievated Graph Key: I112"@en-AU ;
    skos:definition "5 38  Verification of compliance with the Act and other matters"@en-AU ;
    skos:narrower F2021L00304:110 ;
    skos:prefLabel "Item I112"@en-AU ;
    dcat:accessURL <https://www.legislation.gov.au/F2021L00304/asmade/2021-03-24/text/original/epub/OEBPS/document_1/document_1.html#_Toc65844118> ;
    dcat:landingPage "https://www.legislation.gov.au/F2021L00304/asmade/2021-03-24/text/original/epub/OEBPS/document_1/document_1.html#_Toc65844118"^^xsd:anyURI ;
    dcat:theme legcons:Item .

F2021L00304:113 a legcons:Item,
        owl:Class,
        dcat:Resource ;
    rdfs:label "Item - I113 5 39  Action must be taken to address non compliance"@en-AU ;
    dct:isPartOf F2021L00304:110 ;
    dct:isReferencedBy F2021L00304: ;
    rdfs:comment "5 39  Action must be taken to address non compliance - Abrievated Graph Key: I113"@en-AU ;
    skos:definition "5 39  Action must be taken to address non compliance"@en-AU ;
    skos:narrower F2021L00304:110 ;
    skos:prefLabel "Item I113"@en-AU ;
    dcat:accessURL <https://www.legislation.gov.au/F2021L00304/asmade/2021-03-24/text/original/epub/OEBPS/document_1/document_1.html#_Toc65844119> ;
    dcat:landingPage "https://www.legislation.gov.au/F2021L00304/asmade/2021-03-24/text/original/epub/OEBPS/document_1/document_1.html#_Toc65844119"^^xsd:anyURI ;
    dcat:theme legcons:Item .

F2021L00304:114 a legcons:Item,
        owl:Class,
        dcat:Resource ;
    rdfs:label "Item - I114 5 40  Internal audit and management review"@en-AU ;
    dct:isPartOf F2021L00304:110 ;
    dct:isReferencedBy F2021L00304: ;
    rdfs:comment "5 40  Internal audit and management review - Abrievated Graph Key: I114"@en-AU ;
    skos:definition "5 40  Internal audit and management review"@en-AU ;
    skos:narrower F2021L00304:110 ;
    skos:prefLabel "Item I114"@en-AU ;
    dcat:accessURL <https://www.legislation.gov.au/F2021L00304/asmade/2021-03-24/text/original/epub/OEBPS/document_1/document_1.html#_Toc65844120> ;
    dcat:landingPage "https://www.legislation.gov.au/F2021L00304/asmade/2021-03-24/text/original/epub/OEBPS/document_1/document_1.html#_Toc65844120"^^xsd:anyURI ;
    dcat:theme legcons:Item .

F2021L00304:115 a legcons:Item,
        owl:Class,
        dcat:Resource ;
    rdfs:label "Item - I115 5 41  Authorised officer must be notified if prescribed milk or milk products are not fit for human consumption or integrity cannot be ensured etc"@en-AU ;
    dct:isPartOf F2021L00304:110 ;
    dct:isReferencedBy F2021L00304: ;
    rdfs:comment "5 41  Authorised officer must be notified if prescribed milk or milk products are not fit for human consumption or integrity cannot be ensured etc - Abrievated Graph Key: I115"@en-AU ;
    skos:definition "5 41  Authorised officer must be notified if prescribed milk or milk products are not fit for human consumption or integrity cannot be ensured etc"@en-AU ;
    skos:narrower F2021L00304:110 ;
    skos:prefLabel "Item I115"@en-AU ;
    dcat:accessURL <https://www.legislation.gov.au/F2021L00304/asmade/2021-03-24/text/original/epub/OEBPS/document_1/document_1.html#_Toc65844121> ;
    dcat:landingPage "https://www.legislation.gov.au/F2021L00304/asmade/2021-03-24/text/original/epub/OEBPS/document_1/document_1.html#_Toc65844121"^^xsd:anyURI ;
    dcat:theme legcons:Item .

F2021L00304:117 a legcons:Item,
        owl:Class,
        dcat:Resource ;
    rdfs:label "Item - I117 5 42  Period within which application to renew approved arrangement must be made"@en-AU ;
    dct:isPartOf F2021L00304:116 ;
    dct:isReferencedBy F2021L00304: ;
    rdfs:comment "5 42  Period within which application to renew approved arrangement must be made - Abrievated Graph Key: I117"@en-AU ;
    skos:definition "5 42  Period within which application to renew approved arrangement must be made"@en-AU ;
    skos:narrower F2021L00304:116 ;
    skos:prefLabel "Item I117"@en-AU ;
    dcat:accessURL <https://www.legislation.gov.au/F2021L00304/asmade/2021-03-24/text/original/epub/OEBPS/document_1/document_1.html#_Toc65844123> ;
    dcat:landingPage "https://www.legislation.gov.au/F2021L00304/asmade/2021-03-24/text/original/epub/OEBPS/document_1/document_1.html#_Toc65844123"^^xsd:anyURI ;
    dcat:theme legcons:Item .

F2021L00304:120 a legcons:Item,
        owl:Class,
        dcat:Resource ;
    rdfs:label "Item - I120 5 43  Requirements that must be met for variation to be approved or conditions varied"@en-AU ;
    dct:isPartOf F2021L00304:119 ;
    dct:isReferencedBy F2021L00304: ;
    rdfs:comment "5 43  Requirements that must be met for variation to be approved or conditions varied - Abrievated Graph Key: I120"@en-AU ;
    skos:definition "5 43  Requirements that must be met for variation to be approved or conditions varied"@en-AU ;
    skos:narrower F2021L00304:119 ;
    skos:prefLabel "Item I120"@en-AU ;
    dcat:accessURL <https://www.legislation.gov.au/F2021L00304/asmade/2021-03-24/text/original/epub/OEBPS/document_1/document_1.html#_Toc65844126> ;
    dcat:landingPage "https://www.legislation.gov.au/F2021L00304/asmade/2021-03-24/text/original/epub/OEBPS/document_1/document_1.html#_Toc65844126"^^xsd:anyURI ;
    dcat:theme legcons:Item .

F2021L00304:121 a legcons:Item,
        owl:Class,
        dcat:Resource ;
    rdfs:label "Item - I121 5 44  Significant variations"@en-AU ;
    dct:isPartOf F2021L00304:119 ;
    dct:isReferencedBy F2021L00304: ;
    rdfs:comment "5 44  Significant variations - Abrievated Graph Key: I121"@en-AU ;
    skos:definition "5 44  Significant variations"@en-AU ;
    skos:narrower F2021L00304:119 ;
    skos:prefLabel "Item I121"@en-AU ;
    dcat:accessURL <https://www.legislation.gov.au/F2021L00304/asmade/2021-03-24/text/original/epub/OEBPS/document_1/document_1.html#_Toc65844127> ;
    dcat:landingPage "https://www.legislation.gov.au/F2021L00304/asmade/2021-03-24/text/original/epub/OEBPS/document_1/document_1.html#_Toc65844127"^^xsd:anyURI ;
    dcat:theme legcons:Item .

F2021L00304:123 a legcons:Item,
        owl:Class,
        dcat:Resource ;
    rdfs:label "Item - I123 5 45  Other reasons for requiring holder to vary approved arrangement"@en-AU ;
    dct:isPartOf F2021L00304:122 ;
    dct:isReferencedBy F2021L00304: ;
    rdfs:comment "5 45  Other reasons for requiring holder to vary approved arrangement - Abrievated Graph Key: I123"@en-AU ;
    skos:definition "5 45  Other reasons for requiring holder to vary approved arrangement"@en-AU ;
    skos:narrower F2021L00304:122 ;
    skos:prefLabel "Item I123"@en-AU ;
    dcat:accessURL <https://www.legislation.gov.au/F2021L00304/asmade/2021-03-24/text/original/epub/OEBPS/document_1/document_1.html#_Toc65844129> ;
    dcat:landingPage "https://www.legislation.gov.au/F2021L00304/asmade/2021-03-24/text/original/epub/OEBPS/document_1/document_1.html#_Toc65844129"^^xsd:anyURI ;
    dcat:theme legcons:Item .

F2021L00304:125 a legcons:Item,
        owl:Class,
        dcat:Resource ;
    rdfs:label "Item - I125 5 46  Application of this Part"@en-AU ;
    dct:isPartOf F2021L00304:124 ;
    dct:isReferencedBy F2021L00304: ;
    rdfs:comment "5 46  Application of this Part - Abrievated Graph Key: I125"@en-AU ;
    skos:definition "5 46  Application of this Part"@en-AU ;
    skos:narrower F2021L00304:124 ;
    skos:prefLabel "Item I125"@en-AU ;
    dcat:accessURL <https://www.legislation.gov.au/F2021L00304/asmade/2021-03-24/text/original/epub/OEBPS/document_1/document_1.html#_Toc65844131> ;
    dcat:landingPage "https://www.legislation.gov.au/F2021L00304/asmade/2021-03-24/text/original/epub/OEBPS/document_1/document_1.html#_Toc65844131"^^xsd:anyURI ;
    dcat:theme legcons:Item .

F2021L00304:126 a legcons:Item,
        owl:Class,
        dcat:Resource ;
    rdfs:label "Item - I126 5 47  Initial consideration period"@en-AU ;
    dct:isPartOf F2021L00304:124 ;
    dct:isReferencedBy F2021L00304: ;
    rdfs:comment "5 47  Initial consideration period - Abrievated Graph Key: I126"@en-AU ;
    skos:definition "5 47  Initial consideration period"@en-AU ;
    skos:narrower F2021L00304:124 ;
    skos:prefLabel "Item I126"@en-AU ;
    dcat:accessURL <https://www.legislation.gov.au/F2021L00304/asmade/2021-03-24/text/original/epub/OEBPS/document_1/document_1.html#_Toc65844132> ;
    dcat:landingPage "https://www.legislation.gov.au/F2021L00304/asmade/2021-03-24/text/original/epub/OEBPS/document_1/document_1.html#_Toc65844132"^^xsd:anyURI ;
    dcat:theme legcons:Item .

F2021L00304:127 a legcons:Item,
        owl:Class,
        dcat:Resource ;
    rdfs:label "Item - I127 5 48  Period within which request relating to application must be complied with"@en-AU ;
    dct:isPartOf F2021L00304:124 ;
    dct:isReferencedBy F2021L00304: ;
    rdfs:comment "5 48  Period within which request relating to application must be complied with - Abrievated Graph Key: I127"@en-AU ;
    skos:definition "5 48  Period within which request relating to application must be complied with"@en-AU ;
    skos:narrower F2021L00304:124 ;
    skos:prefLabel "Item I127"@en-AU ;
    dcat:accessURL <https://www.legislation.gov.au/F2021L00304/asmade/2021-03-24/text/original/epub/OEBPS/document_1/document_1.html#_Toc65844133> ;
    dcat:landingPage "https://www.legislation.gov.au/F2021L00304/asmade/2021-03-24/text/original/epub/OEBPS/document_1/document_1.html#_Toc65844133"^^xsd:anyURI ;
    dcat:theme legcons:Item .

F2021L00304:13 a legcons:Item,
        owl:Class,
        dcat:Resource ;
    rdfs:label "Item - I13 2 1  Milk and milk products that are prescribed goods"@en-AU ;
    dct:isPartOf F2021L00304:12 ;
    dct:isReferencedBy F2021L00304: ;
    rdfs:comment "2 1  Milk and milk products that are prescribed goods - Abrievated Graph Key: I13"@en-AU ;
    skos:definition "2 1  Milk and milk products that are prescribed goods"@en-AU ;
    skos:narrower F2021L00304:12 ;
    skos:prefLabel "Item I13"@en-AU ;
    dcat:accessURL <https://www.legislation.gov.au/F2021L00304/asmade/2021-03-24/text/original/epub/OEBPS/document_1/document_1.html#_Toc65844019> ;
    dcat:landingPage "https://www.legislation.gov.au/F2021L00304/asmade/2021-03-24/text/original/epub/OEBPS/document_1/document_1.html#_Toc65844019"^^xsd:anyURI ;
    dcat:theme legcons:Item .

F2021L00304:130 a legcons:Item,
        owl:Class,
        dcat:Resource ;
    rdfs:label "Item - I130 7 1  Conditions of export permit"@en-AU ;
    dct:isPartOf F2021L00304:129 ;
    dct:isReferencedBy F2021L00304: ;
    rdfs:comment "7 1  Conditions of export permit - Abrievated Graph Key: I130"@en-AU ;
    skos:definition "7 1  Conditions of export permit"@en-AU ;
    skos:narrower F2021L00304:129 ;
    skos:prefLabel "Item I130"@en-AU ;
    dcat:accessURL <https://www.legislation.gov.au/F2021L00304/asmade/2021-03-24/text/original/epub/OEBPS/document_1/document_1.html#_Toc65844136> ;
    dcat:landingPage "https://www.legislation.gov.au/F2021L00304/asmade/2021-03-24/text/original/epub/OEBPS/document_1/document_1.html#_Toc65844136"^^xsd:anyURI ;
    dcat:theme legcons:Item .

F2021L00304:131 a legcons:Item,
        owl:Class,
        dcat:Resource ;
    rdfs:label "Item - I131 7 2  Period of effect of export permit"@en-AU ;
    dct:isPartOf F2021L00304:129 ;
    dct:isReferencedBy F2021L00304: ;
    rdfs:comment "7 2  Period of effect of export permit - Abrievated Graph Key: I131"@en-AU ;
    skos:definition "7 2  Period of effect of export permit"@en-AU ;
    skos:narrower F2021L00304:129 ;
    skos:prefLabel "Item I131"@en-AU ;
    dcat:accessURL <https://www.legislation.gov.au/F2021L00304/asmade/2021-03-24/text/original/epub/OEBPS/document_1/document_1.html#_Toc65844137> ;
    dcat:landingPage "https://www.legislation.gov.au/F2021L00304/asmade/2021-03-24/text/original/epub/OEBPS/document_1/document_1.html#_Toc65844137"^^xsd:anyURI ;
    dcat:theme legcons:Item .

F2021L00304:133 a legcons:Item,
        owl:Class,
        dcat:Resource ;
    rdfs:label "Item - I133 7 3  Period of effect of varied export permit"@en-AU ;
    dct:isPartOf F2021L00304:132 ;
    dct:isReferencedBy F2021L00304: ;
    rdfs:comment "7 3  Period of effect of varied export permit - Abrievated Graph Key: I133"@en-AU ;
    skos:definition "7 3  Period of effect of varied export permit"@en-AU ;
    skos:narrower F2021L00304:132 ;
    skos:prefLabel "Item I133"@en-AU ;
    dcat:accessURL <https://www.legislation.gov.au/F2021L00304/asmade/2021-03-24/text/original/epub/OEBPS/document_1/document_1.html#_Toc65844139> ;
    dcat:landingPage "https://www.legislation.gov.au/F2021L00304/asmade/2021-03-24/text/original/epub/OEBPS/document_1/document_1.html#_Toc65844139"^^xsd:anyURI ;
    dcat:theme legcons:Item .

F2021L00304:134 a legcons:Item,
        owl:Class,
        dcat:Resource ;
    rdfs:label "Item - I134 7 4  Circumstances in which export permit may be suspended"@en-AU ;
    dct:isPartOf F2021L00304:132 ;
    dct:isReferencedBy F2021L00304: ;
    rdfs:comment "7 4  Circumstances in which export permit may be suspended - Abrievated Graph Key: I134"@en-AU ;
    skos:definition "7 4  Circumstances in which export permit may be suspended"@en-AU ;
    skos:narrower F2021L00304:132 ;
    skos:prefLabel "Item I134"@en-AU ;
    dcat:accessURL <https://www.legislation.gov.au/F2021L00304/asmade/2021-03-24/text/original/epub/OEBPS/document_1/document_1.html#_Toc65844140> ;
    dcat:landingPage "https://www.legislation.gov.au/F2021L00304/asmade/2021-03-24/text/original/epub/OEBPS/document_1/document_1.html#_Toc65844140"^^xsd:anyURI ;
    dcat:theme legcons:Item .

F2021L00304:135 a legcons:Item,
        owl:Class,
        dcat:Resource ;
    rdfs:label "Item - I135 7 5  Other circumstances in which export permit may be revoked"@en-AU ;
    dct:isPartOf F2021L00304:132 ;
    dct:isReferencedBy F2021L00304: ;
    rdfs:comment "7 5  Other circumstances in which export permit may be revoked - Abrievated Graph Key: I135"@en-AU ;
    skos:definition "7 5  Other circumstances in which export permit may be revoked"@en-AU ;
    skos:narrower F2021L00304:132 ;
    skos:prefLabel "Item I135"@en-AU ;
    dcat:accessURL <https://www.legislation.gov.au/F2021L00304/asmade/2021-03-24/text/original/epub/OEBPS/document_1/document_1.html#_Toc65844141> ;
    dcat:landingPage "https://www.legislation.gov.au/F2021L00304/asmade/2021-03-24/text/original/epub/OEBPS/document_1/document_1.html#_Toc65844141"^^xsd:anyURI ;
    dcat:theme legcons:Item .

F2021L00304:137 a legcons:Item,
        owl:Class,
        dcat:Resource ;
    rdfs:label "Item - I137 7 6  Changes that require additional or corrected information to be given to the Secretary"@en-AU ;
    dct:isPartOf F2021L00304:136 ;
    dct:isReferencedBy F2021L00304: ;
    rdfs:comment "7 6  Changes that require additional or corrected information to be given to the Secretary - Abrievated Graph Key: I137"@en-AU ;
    skos:definition "7 6  Changes that require additional or corrected information to be given to the Secretary"@en-AU ;
    skos:narrower F2021L00304:136 ;
    skos:prefLabel "Item I137"@en-AU ;
    dcat:accessURL <https://www.legislation.gov.au/F2021L00304/asmade/2021-03-24/text/original/epub/OEBPS/document_1/document_1.html#_Toc65844143> ;
    dcat:landingPage "https://www.legislation.gov.au/F2021L00304/asmade/2021-03-24/text/original/epub/OEBPS/document_1/document_1.html#_Toc65844143"^^xsd:anyURI ;
    dcat:theme legcons:Item .

F2021L00304:138 a legcons:Item,
        owl:Class,
        dcat:Resource ;
    rdfs:label "Item - I138 7 7  Return of export permit"@en-AU ;
    dct:isPartOf F2021L00304:136 ;
    dct:isReferencedBy F2021L00304: ;
    rdfs:comment "7 7  Return of export permit - Abrievated Graph Key: I138"@en-AU ;
    skos:definition "7 7  Return of export permit"@en-AU ;
    skos:narrower F2021L00304:136 ;
    skos:prefLabel "Item I138"@en-AU ;
    dcat:accessURL <https://www.legislation.gov.au/F2021L00304/asmade/2021-03-24/text/original/epub/OEBPS/document_1/document_1.html#_Toc65844144> ;
    dcat:landingPage "https://www.legislation.gov.au/F2021L00304/asmade/2021-03-24/text/original/epub/OEBPS/document_1/document_1.html#_Toc65844144"^^xsd:anyURI ;
    dcat:theme legcons:Item .

F2021L00304:139 a legcons:Item,
        owl:Class,
        dcat:Resource ;
    rdfs:label "Item - I139 7 8  Notification that prescribed milk or milk products are not to be exported"@en-AU ;
    dct:isPartOf F2021L00304:136 ;
    dct:isReferencedBy F2021L00304: ;
    rdfs:comment "7 8  Notification that prescribed milk or milk products are not to be exported - Abrievated Graph Key: I139"@en-AU ;
    skos:definition "7 8  Notification that prescribed milk or milk products are not to be exported"@en-AU ;
    skos:narrower F2021L00304:136 ;
    skos:prefLabel "Item I139"@en-AU ;
    dcat:accessURL <https://www.legislation.gov.au/F2021L00304/asmade/2021-03-24/text/original/epub/OEBPS/document_1/document_1.html#_Toc65844145> ;
    dcat:landingPage "https://www.legislation.gov.au/F2021L00304/asmade/2021-03-24/text/original/epub/OEBPS/document_1/document_1.html#_Toc65844145"^^xsd:anyURI ;
    dcat:theme legcons:Item .

F2021L00304:14 a legcons:Item,
        owl:Class,
        dcat:Resource ;
    rdfs:label "Item - I14 2 2  Milk and milk products that are taken not to be prescribed goods"@en-AU ;
    dct:isPartOf F2021L00304:12 ;
    dct:isReferencedBy F2021L00304: ;
    rdfs:comment "2 2  Milk and milk products that are taken not to be prescribed goods - Abrievated Graph Key: I14"@en-AU ;
    skos:definition "2 2  Milk and milk products that are taken not to be prescribed goods"@en-AU ;
    skos:narrower F2021L00304:12 ;
    skos:prefLabel "Item I14"@en-AU ;
    dcat:accessURL <https://www.legislation.gov.au/F2021L00304/asmade/2021-03-24/text/original/epub/OEBPS/document_1/document_1.html#_Toc65844020> ;
    dcat:landingPage "https://www.legislation.gov.au/F2021L00304/asmade/2021-03-24/text/original/epub/OEBPS/document_1/document_1.html#_Toc65844020"^^xsd:anyURI ;
    dcat:theme legcons:Item .

F2021L00304:141 a legcons:Item,
        owl:Class,
        dcat:Resource ;
    rdfs:label "Item - I141 7 9  Application of this Part"@en-AU ;
    dct:isPartOf F2021L00304:140 ;
    dct:isReferencedBy F2021L00304: ;
    rdfs:comment "7 9  Application of this Part - Abrievated Graph Key: I141"@en-AU ;
    skos:definition "7 9  Application of this Part"@en-AU ;
    skos:narrower F2021L00304:140 ;
    skos:prefLabel "Item I141"@en-AU ;
    dcat:accessURL <https://www.legislation.gov.au/F2021L00304/asmade/2021-03-24/text/original/epub/OEBPS/document_1/document_1.html#_Toc65844147> ;
    dcat:landingPage "https://www.legislation.gov.au/F2021L00304/asmade/2021-03-24/text/original/epub/OEBPS/document_1/document_1.html#_Toc65844147"^^xsd:anyURI ;
    dcat:theme legcons:Item .

F2021L00304:142 a legcons:Item,
        owl:Class,
        dcat:Resource ;
    rdfs:label "Item - I142 7 10  Documents to accompany application"@en-AU ;
    dct:isPartOf F2021L00304:140 ;
    dct:isReferencedBy F2021L00304: ;
    rdfs:comment "7 10  Documents to accompany application - Abrievated Graph Key: I142"@en-AU ;
    skos:definition "7 10  Documents to accompany application"@en-AU ;
    skos:narrower F2021L00304:140 ;
    skos:prefLabel "Item I142"@en-AU ;
    dcat:accessURL <https://www.legislation.gov.au/F2021L00304/asmade/2021-03-24/text/original/epub/OEBPS/document_1/document_1.html#_Toc65844148> ;
    dcat:landingPage "https://www.legislation.gov.au/F2021L00304/asmade/2021-03-24/text/original/epub/OEBPS/document_1/document_1.html#_Toc65844148"^^xsd:anyURI ;
    dcat:theme legcons:Item .

F2021L00304:145 a legcons:Item,
        owl:Class,
        dcat:Resource ;
    rdfs:label "Item - I145 8 1  Purpose of this Part"@en-AU ;
    dct:isPartOf F2021L00304:144 ;
    dct:isReferencedBy F2021L00304: ;
    rdfs:comment "8 1  Purpose of this Part - Abrievated Graph Key: I145"@en-AU ;
    skos:definition "8 1  Purpose of this Part"@en-AU ;
    skos:narrower F2021L00304:144 ;
    skos:prefLabel "Item I145"@en-AU ;
    dcat:accessURL <https://www.legislation.gov.au/F2021L00304/asmade/2021-03-24/text/original/epub/OEBPS/document_1/document_1.html#_Toc65844151> ;
    dcat:landingPage "https://www.legislation.gov.au/F2021L00304/asmade/2021-03-24/text/original/epub/OEBPS/document_1/document_1.html#_Toc65844151"^^xsd:anyURI ;
    dcat:theme legcons:Item .

F2021L00304:146 a legcons:Item,
        owl:Class,
        dcat:Resource ;
    rdfs:label "Item - I146 8 2  General requirements for trade descriptions"@en-AU ;
    dct:isPartOf F2021L00304:144 ;
    dct:isReferencedBy F2021L00304: ;
    rdfs:comment "8 2  General requirements for trade descriptions - Abrievated Graph Key: I146"@en-AU ;
    skos:definition "8 2  General requirements for trade descriptions"@en-AU ;
    skos:narrower F2021L00304:144 ;
    skos:prefLabel "Item I146"@en-AU ;
    dcat:accessURL <https://www.legislation.gov.au/F2021L00304/asmade/2021-03-24/text/original/epub/OEBPS/document_1/document_1.html#_Toc65844152> ;
    dcat:landingPage "https://www.legislation.gov.au/F2021L00304/asmade/2021-03-24/text/original/epub/OEBPS/document_1/document_1.html#_Toc65844152"^^xsd:anyURI ;
    dcat:theme legcons:Item .

F2021L00304:147 a legcons:Item,
        owl:Class,
        dcat:Resource ;
    rdfs:label "Item - I147 8 3  Trade descriptions in language other than English"@en-AU ;
    dct:isPartOf F2021L00304:144 ;
    dct:isReferencedBy F2021L00304: ;
    rdfs:comment "8 3  Trade descriptions in language other than English - Abrievated Graph Key: I147"@en-AU ;
    skos:definition "8 3  Trade descriptions in language other than English"@en-AU ;
    skos:narrower F2021L00304:144 ;
    skos:prefLabel "Item I147"@en-AU ;
    dcat:accessURL <https://www.legislation.gov.au/F2021L00304/asmade/2021-03-24/text/original/epub/OEBPS/document_1/document_1.html#_Toc65844153> ;
    dcat:landingPage "https://www.legislation.gov.au/F2021L00304/asmade/2021-03-24/text/original/epub/OEBPS/document_1/document_1.html#_Toc65844153"^^xsd:anyURI ;
    dcat:theme legcons:Item .

F2021L00304:15 a legcons:Division,
        owl:Class,
        dcat:Resource ;
    rdfs:label "Division - D15 Division 2 Prohibited export and prescribed export conditions"@en-AU ;
    dct:isPartOf F2021L00304:11 ;
    dct:isReferencedBy F2021L00304: ;
    rdfs:comment "Division 2 Prohibited export and prescribed export conditions - Abrievated Graph Key: D15"@en-AU ;
    skos:definition "Division 2 Prohibited export and prescribed export conditions"@en-AU ;
    skos:narrower F2021L00304:11 ;
    skos:prefLabel "Division D15"@en-AU ;
    dcat:accessURL <https://www.legislation.gov.au/F2021L00304/asmade/2021-03-24/text/original/epub/OEBPS/document_1/document_1.html#_Toc65844021> ;
    dcat:landingPage "https://www.legislation.gov.au/F2021L00304/asmade/2021-03-24/text/original/epub/OEBPS/document_1/document_1.html#_Toc65844021"^^xsd:anyURI ;
    dcat:theme legcons:Division .

F2021L00304:150 a legcons:Item,
        owl:Class,
        dcat:Resource ;
    rdfs:label "Item - I150 8 4  Purpose of this Division"@en-AU ;
    dct:isPartOf F2021L00304:149 ;
    dct:isReferencedBy F2021L00304: ;
    rdfs:comment "8 4  Purpose of this Division - Abrievated Graph Key: I150"@en-AU ;
    skos:definition "8 4  Purpose of this Division"@en-AU ;
    skos:narrower F2021L00304:149 ;
    skos:prefLabel "Item I150"@en-AU ;
    dcat:accessURL <https://www.legislation.gov.au/F2021L00304/asmade/2021-03-24/text/original/epub/OEBPS/document_1/document_1.html#_Toc65844156> ;
    dcat:landingPage "https://www.legislation.gov.au/F2021L00304/asmade/2021-03-24/text/original/epub/OEBPS/document_1/document_1.html#_Toc65844156"^^xsd:anyURI ;
    dcat:theme legcons:Item .

F2021L00304:151 a legcons:Item,
        owl:Class,
        dcat:Resource ;
    rdfs:label "Item - I151 8 5  Tolerances for dimensions of official marks"@en-AU ;
    dct:isPartOf F2021L00304:149 ;
    dct:isReferencedBy F2021L00304: ;
    rdfs:comment "8 5  Tolerances for dimensions of official marks - Abrievated Graph Key: I151"@en-AU ;
    skos:definition "8 5  Tolerances for dimensions of official marks"@en-AU ;
    skos:narrower F2021L00304:149 ;
    skos:prefLabel "Item I151"@en-AU ;
    dcat:accessURL <https://www.legislation.gov.au/F2021L00304/asmade/2021-03-24/text/original/epub/OEBPS/document_1/document_1.html#_Toc65844157> ;
    dcat:landingPage "https://www.legislation.gov.au/F2021L00304/asmade/2021-03-24/text/original/epub/OEBPS/document_1/document_1.html#_Toc65844157"^^xsd:anyURI ;
    dcat:theme legcons:Item .

F2021L00304:152 a legcons:Item,
        owl:Class,
        dcat:Resource ;
    rdfs:label "Item - I152 8 6  Official markforeign country identification"@en-AU ;
    dct:isPartOf F2021L00304:149 ;
    dct:isReferencedBy F2021L00304: ;
    rdfs:comment "8 6  Official markforeign country identification - Abrievated Graph Key: I152"@en-AU ;
    skos:definition "8 6  Official markforeign country identification"@en-AU ;
    skos:narrower F2021L00304:149 ;
    skos:prefLabel "Item I152"@en-AU ;
    dcat:accessURL <https://www.legislation.gov.au/F2021L00304/asmade/2021-03-24/text/original/epub/OEBPS/document_1/document_1.html#_Toc65844158> ;
    dcat:landingPage "https://www.legislation.gov.au/F2021L00304/asmade/2021-03-24/text/original/epub/OEBPS/document_1/document_1.html#_Toc65844158"^^xsd:anyURI ;
    dcat:theme legcons:Item .

F2021L00304:153 a legcons:Item,
        owl:Class,
        dcat:Resource ;
    rdfs:label "Item - I153 8 7  Official marktamper indicative metal strap seal"@en-AU ;
    dct:isPartOf F2021L00304:149 ;
    dct:isReferencedBy F2021L00304: ;
    rdfs:comment "8 7  Official marktamper indicative metal strap seal - Abrievated Graph Key: I153"@en-AU ;
    skos:definition "8 7  Official marktamper indicative metal strap seal"@en-AU ;
    skos:narrower F2021L00304:149 ;
    skos:prefLabel "Item I153"@en-AU ;
    dcat:accessURL <https://www.legislation.gov.au/F2021L00304/asmade/2021-03-24/text/original/epub/OEBPS/document_1/document_1.html#_Toc65844159> ;
    dcat:landingPage "https://www.legislation.gov.au/F2021L00304/asmade/2021-03-24/text/original/epub/OEBPS/document_1/document_1.html#_Toc65844159"^^xsd:anyURI ;
    dcat:theme legcons:Item .

F2021L00304:154 a legcons:Item,
        owl:Class,
        dcat:Resource ;
    rdfs:label "Item - I154 8 8  Official markbolt seal"@en-AU ;
    dct:isPartOf F2021L00304:149 ;
    dct:isReferencedBy F2021L00304: ;
    rdfs:comment "8 8  Official markbolt seal - Abrievated Graph Key: I154"@en-AU ;
    skos:definition "8 8  Official markbolt seal"@en-AU ;
    skos:narrower F2021L00304:149 ;
    skos:prefLabel "Item I154"@en-AU ;
    dcat:accessURL <https://www.legislation.gov.au/F2021L00304/asmade/2021-03-24/text/original/epub/OEBPS/document_1/document_1.html#_Toc65844160> ;
    dcat:landingPage "https://www.legislation.gov.au/F2021L00304/asmade/2021-03-24/text/original/epub/OEBPS/document_1/document_1.html#_Toc65844160"^^xsd:anyURI ;
    dcat:theme legcons:Item .

F2021L00304:155 a legcons:Item,
        owl:Class,
        dcat:Resource ;
    rdfs:label "Item - I155 8 9  Official markEuropean Union"@en-AU ;
    dct:isPartOf F2021L00304:149 ;
    dct:isReferencedBy F2021L00304: ;
    rdfs:comment "8 9  Official markEuropean Union - Abrievated Graph Key: I155"@en-AU ;
    skos:definition "8 9  Official markEuropean Union"@en-AU ;
    skos:narrower F2021L00304:149 ;
    skos:prefLabel "Item I155"@en-AU ;
    dcat:accessURL <https://www.legislation.gov.au/F2021L00304/asmade/2021-03-24/text/original/epub/OEBPS/document_1/document_1.html#_Toc65844161> ;
    dcat:landingPage "https://www.legislation.gov.au/F2021L00304/asmade/2021-03-24/text/original/epub/OEBPS/document_1/document_1.html#_Toc65844161"^^xsd:anyURI ;
    dcat:theme legcons:Item .

F2021L00304:156 a legcons:Item,
        owl:Class,
        dcat:Resource ;
    rdfs:label "Item - I156 8 10  Official markcarton seal"@en-AU ;
    dct:isPartOf F2021L00304:149 ;
    dct:isReferencedBy F2021L00304: ;
    rdfs:comment "8 10  Official markcarton seal - Abrievated Graph Key: I156"@en-AU ;
    skos:definition "8 10  Official markcarton seal"@en-AU ;
    skos:narrower F2021L00304:149 ;
    skos:prefLabel "Item I156"@en-AU ;
    dcat:accessURL <https://www.legislation.gov.au/F2021L00304/asmade/2021-03-24/text/original/epub/OEBPS/document_1/document_1.html#_Toc65844162> ;
    dcat:landingPage "https://www.legislation.gov.au/F2021L00304/asmade/2021-03-24/text/original/epub/OEBPS/document_1/document_1.html#_Toc65844162"^^xsd:anyURI ;
    dcat:theme legcons:Item .

F2021L00304:157 a legcons:Item,
        owl:Class,
        dcat:Resource ;
    rdfs:label "Item - I157 8 11  Official markgoods opened for assessment and resealed"@en-AU ;
    dct:isPartOf F2021L00304:149 ;
    dct:isReferencedBy F2021L00304: ;
    rdfs:comment "8 11  Official markgoods opened for assessment and resealed - Abrievated Graph Key: I157"@en-AU ;
    skos:definition "8 11  Official markgoods opened for assessment and resealed"@en-AU ;
    skos:narrower F2021L00304:149 ;
    skos:prefLabel "Item I157"@en-AU ;
    dcat:accessURL <https://www.legislation.gov.au/F2021L00304/asmade/2021-03-24/text/original/epub/OEBPS/document_1/document_1.html#_Toc65844163> ;
    dcat:landingPage "https://www.legislation.gov.au/F2021L00304/asmade/2021-03-24/text/original/epub/OEBPS/document_1/document_1.html#_Toc65844163"^^xsd:anyURI ;
    dcat:theme legcons:Item .

F2021L00304:158 a legcons:Item,
        owl:Class,
        dcat:Resource ;
    rdfs:label "Item - I158 8 12  Official markAustralian Government"@en-AU ;
    dct:isPartOf F2021L00304:149 ;
    dct:isReferencedBy F2021L00304: ;
    rdfs:comment "8 12  Official markAustralian Government - Abrievated Graph Key: I158"@en-AU ;
    skos:definition "8 12  Official markAustralian Government"@en-AU ;
    skos:narrower F2021L00304:149 ;
    skos:prefLabel "Item I158"@en-AU ;
    dcat:accessURL <https://www.legislation.gov.au/F2021L00304/asmade/2021-03-24/text/original/epub/OEBPS/document_1/document_1.html#_Toc65844164> ;
    dcat:landingPage "https://www.legislation.gov.au/F2021L00304/asmade/2021-03-24/text/original/epub/OEBPS/document_1/document_1.html#_Toc65844164"^^xsd:anyURI ;
    dcat:theme legcons:Item .

F2021L00304:16 a legcons:Item,
        owl:Class,
        dcat:Resource ;
    rdfs:label "Item - I16 2 3  Purpose and application of this Division"@en-AU ;
    dct:isPartOf F2021L00304:11 ;
    dct:isReferencedBy F2021L00304: ;
    rdfs:comment "2 3  Purpose and application of this Division - Abrievated Graph Key: I16"@en-AU ;
    skos:definition "2 3  Purpose and application of this Division"@en-AU ;
    skos:narrower F2021L00304:11 ;
    skos:prefLabel "Item I16"@en-AU ;
    dcat:accessURL <https://www.legislation.gov.au/F2021L00304/asmade/2021-03-24/text/original/epub/OEBPS/document_1/document_1.html#_Toc65844022> ;
    dcat:landingPage "https://www.legislation.gov.au/F2021L00304/asmade/2021-03-24/text/original/epub/OEBPS/document_1/document_1.html#_Toc65844022"^^xsd:anyURI ;
    dcat:theme legcons:Item .

F2021L00304:160 a legcons:Item,
        owl:Class,
        dcat:Resource ;
    rdfs:label "Item - I160 8 13  Purpose and application of this Division"@en-AU ;
    dct:isPartOf F2021L00304:159 ;
    dct:isReferencedBy F2021L00304: ;
    rdfs:comment "8 13  Purpose and application of this Division - Abrievated Graph Key: I160"@en-AU ;
    skos:definition "8 13  Purpose and application of this Division"@en-AU ;
    skos:narrower F2021L00304:159 ;
    skos:prefLabel "Item I160"@en-AU ;
    dcat:accessURL <https://www.legislation.gov.au/F2021L00304/asmade/2021-03-24/text/original/epub/OEBPS/document_1/document_1.html#_Toc65844166> ;
    dcat:landingPage "https://www.legislation.gov.au/F2021L00304/asmade/2021-03-24/text/original/epub/OEBPS/document_1/document_1.html#_Toc65844166"^^xsd:anyURI ;
    dcat:theme legcons:Item .

F2021L00304:161 a legcons:Item,
        owl:Class,
        dcat:Resource ;
    rdfs:label "Item - I161 8 14  Interpretation"@en-AU ;
    dct:isPartOf F2021L00304:159 ;
    dct:isReferencedBy F2021L00304: ;
    rdfs:comment "8 14  Interpretation - Abrievated Graph Key: I161"@en-AU ;
    skos:definition "8 14  Interpretation"@en-AU ;
    skos:narrower F2021L00304:159 ;
    skos:prefLabel "Item I161"@en-AU ;
    dcat:accessURL <https://www.legislation.gov.au/F2021L00304/asmade/2021-03-24/text/original/epub/OEBPS/document_1/document_1.html#_Toc65844167> ;
    dcat:landingPage "https://www.legislation.gov.au/F2021L00304/asmade/2021-03-24/text/original/epub/OEBPS/document_1/document_1.html#_Toc65844167"^^xsd:anyURI ;
    dcat:theme legcons:Item .

F2021L00304:162 a legcons:Item,
        owl:Class,
        dcat:Resource ;
    rdfs:label "Item - I162 8 15  Persons who may manufacture or supply official marks for milk or milk products"@en-AU ;
    dct:isPartOf F2021L00304:159 ;
    dct:isReferencedBy F2021L00304: ;
    rdfs:comment "8 15  Persons who may manufacture or supply official marks for milk or milk products - Abrievated Graph Key: I162"@en-AU ;
    skos:definition "8 15  Persons who may manufacture or supply official marks for milk or milk products"@en-AU ;
    skos:narrower F2021L00304:159 ;
    skos:prefLabel "Item I162"@en-AU ;
    dcat:accessURL <https://www.legislation.gov.au/F2021L00304/asmade/2021-03-24/text/original/epub/OEBPS/document_1/document_1.html#_Toc65844168> ;
    dcat:landingPage "https://www.legislation.gov.au/F2021L00304/asmade/2021-03-24/text/original/epub/OEBPS/document_1/document_1.html#_Toc65844168"^^xsd:anyURI ;
    dcat:theme legcons:Item .

F2021L00304:163 a legcons:Item,
        owl:Class,
        dcat:Resource ;
    rdfs:label "Item - I163 8 16  Persons who may possess official marks that have not been applied to milk or milk products"@en-AU ;
    dct:isPartOf F2021L00304:159 ;
    dct:isReferencedBy F2021L00304: ;
    rdfs:comment "8 16  Persons who may possess official marks that have not been applied to milk or milk products - Abrievated Graph Key: I163"@en-AU ;
    skos:definition "8 16  Persons who may possess official marks that have not been applied to milk or milk products"@en-AU ;
    skos:narrower F2021L00304:159 ;
    skos:prefLabel "Item I163"@en-AU ;
    dcat:accessURL <https://www.legislation.gov.au/F2021L00304/asmade/2021-03-24/text/original/epub/OEBPS/document_1/document_1.html#_Toc65844169> ;
    dcat:landingPage "https://www.legislation.gov.au/F2021L00304/asmade/2021-03-24/text/original/epub/OEBPS/document_1/document_1.html#_Toc65844169"^^xsd:anyURI ;
    dcat:theme legcons:Item .

F2021L00304:164 a legcons:Item,
        owl:Class,
        dcat:Resource ;
    rdfs:label "Item - I164 8 17  Persons who may apply official marks to milk or milk products etc"@en-AU ;
    dct:isPartOf F2021L00304:159 ;
    dct:isReferencedBy F2021L00304: ;
    rdfs:comment "8 17  Persons who may apply official marks to milk or milk products etc - Abrievated Graph Key: I164"@en-AU ;
    skos:definition "8 17  Persons who may apply official marks to milk or milk products etc"@en-AU ;
    skos:narrower F2021L00304:159 ;
    skos:prefLabel "Item I164"@en-AU ;
    dcat:accessURL <https://www.legislation.gov.au/F2021L00304/asmade/2021-03-24/text/original/epub/OEBPS/document_1/document_1.html#_Toc65844170> ;
    dcat:landingPage "https://www.legislation.gov.au/F2021L00304/asmade/2021-03-24/text/original/epub/OEBPS/document_1/document_1.html#_Toc65844170"^^xsd:anyURI ;
    dcat:theme legcons:Item .

F2021L00304:165 a legcons:Item,
        owl:Class,
        dcat:Resource ;
    rdfs:label "Item - I165 8 18  Circumstances in which official mark must not be applied to milk or milk products"@en-AU ;
    dct:isPartOf F2021L00304:159 ;
    dct:isReferencedBy F2021L00304: ;
    rdfs:comment "8 18  Circumstances in which official mark must not be applied to milk or milk products - Abrievated Graph Key: I165"@en-AU ;
    skos:definition "8 18  Circumstances in which official mark must not be applied to milk or milk products"@en-AU ;
    skos:narrower F2021L00304:159 ;
    skos:prefLabel "Item I165"@en-AU ;
    dcat:accessURL <https://www.legislation.gov.au/F2021L00304/asmade/2021-03-24/text/original/epub/OEBPS/document_1/document_1.html#_Toc65844171> ;
    dcat:landingPage "https://www.legislation.gov.au/F2021L00304/asmade/2021-03-24/text/original/epub/OEBPS/document_1/document_1.html#_Toc65844171"^^xsd:anyURI ;
    dcat:theme legcons:Item .

F2021L00304:166 a legcons:Item,
        owl:Class,
        dcat:Resource ;
    rdfs:label "Item - I166 8 19  Alteration of and interference with official marks"@en-AU ;
    dct:isPartOf F2021L00304:159 ;
    dct:isReferencedBy F2021L00304: ;
    rdfs:comment "8 19  Alteration of and interference with official marks - Abrievated Graph Key: I166"@en-AU ;
    skos:definition "8 19  Alteration of and interference with official marks"@en-AU ;
    skos:narrower F2021L00304:159 ;
    skos:prefLabel "Item I166"@en-AU ;
    dcat:accessURL <https://www.legislation.gov.au/F2021L00304/asmade/2021-03-24/text/original/epub/OEBPS/document_1/document_1.html#_Toc65844172> ;
    dcat:landingPage "https://www.legislation.gov.au/F2021L00304/asmade/2021-03-24/text/original/epub/OEBPS/document_1/document_1.html#_Toc65844172"^^xsd:anyURI ;
    dcat:theme legcons:Item .

F2021L00304:167 a legcons:Item,
        owl:Class,
        dcat:Resource ;
    rdfs:label "Item - I167 8 20  Official marks must be legible and securely attached"@en-AU ;
    dct:isPartOf F2021L00304:159 ;
    dct:isReferencedBy F2021L00304: ;
    rdfs:comment "8 20  Official marks must be legible and securely attached - Abrievated Graph Key: I167"@en-AU ;
    skos:definition "8 20  Official marks must be legible and securely attached"@en-AU ;
    skos:narrower F2021L00304:159 ;
    skos:prefLabel "Item I167"@en-AU ;
    dcat:accessURL <https://www.legislation.gov.au/F2021L00304/asmade/2021-03-24/text/original/epub/OEBPS/document_1/document_1.html#_Toc65844173> ;
    dcat:landingPage "https://www.legislation.gov.au/F2021L00304/asmade/2021-03-24/text/original/epub/OEBPS/document_1/document_1.html#_Toc65844173"^^xsd:anyURI ;
    dcat:theme legcons:Item .

F2021L00304:168 a legcons:Item,
        owl:Class,
        dcat:Resource ;
    rdfs:label "Item - I168 8 21  Security of official marks"@en-AU ;
    dct:isPartOf F2021L00304:159 ;
    dct:isReferencedBy F2021L00304: ;
    rdfs:comment "8 21  Security of official marks - Abrievated Graph Key: I168"@en-AU ;
    skos:definition "8 21  Security of official marks"@en-AU ;
    skos:narrower F2021L00304:159 ;
    skos:prefLabel "Item I168"@en-AU ;
    dcat:accessURL <https://www.legislation.gov.au/F2021L00304/asmade/2021-03-24/text/original/epub/OEBPS/document_1/document_1.html#_Toc65844174> ;
    dcat:landingPage "https://www.legislation.gov.au/F2021L00304/asmade/2021-03-24/text/original/epub/OEBPS/document_1/document_1.html#_Toc65844174"^^xsd:anyURI ;
    dcat:theme legcons:Item .

F2021L00304:169 a legcons:Item,
        owl:Class,
        dcat:Resource ;
    rdfs:label "Item - I169 8 22  Removal or defacement of official marks"@en-AU ;
    dct:isPartOf F2021L00304:159 ;
    dct:isReferencedBy F2021L00304: ;
    rdfs:comment "8 22  Removal or defacement of official marks - Abrievated Graph Key: I169"@en-AU ;
    skos:definition "8 22  Removal or defacement of official marks"@en-AU ;
    skos:narrower F2021L00304:159 ;
    skos:prefLabel "Item I169"@en-AU ;
    dcat:accessURL <https://www.legislation.gov.au/F2021L00304/asmade/2021-03-24/text/original/epub/OEBPS/document_1/document_1.html#_Toc65844175> ;
    dcat:landingPage "https://www.legislation.gov.au/F2021L00304/asmade/2021-03-24/text/original/epub/OEBPS/document_1/document_1.html#_Toc65844175"^^xsd:anyURI ;
    dcat:theme legcons:Item .

F2021L00304:17 a legcons:Item,
        owl:Class,
        dcat:Resource ;
    rdfs:label "Item - I17 2 4  Export of prescribed milk or milk products is prohibited unless prescribed conditions are complied with"@en-AU ;
    dct:isPartOf F2021L00304:11 ;
    dct:isReferencedBy F2021L00304: ;
    rdfs:comment "2 4  Export of prescribed milk or milk products is prohibited unless prescribed conditions are complied with - Abrievated Graph Key: I17"@en-AU ;
    skos:definition "2 4  Export of prescribed milk or milk products is prohibited unless prescribed conditions are complied with"@en-AU ;
    skos:narrower F2021L00304:11 ;
    skos:prefLabel "Item I17"@en-AU ;
    dcat:accessURL <https://www.legislation.gov.au/F2021L00304/asmade/2021-03-24/text/original/epub/OEBPS/document_1/document_1.html#_Toc65844023> ;
    dcat:landingPage "https://www.legislation.gov.au/F2021L00304/asmade/2021-03-24/text/original/epub/OEBPS/document_1/document_1.html#_Toc65844023"^^xsd:anyURI ;
    dcat:theme legcons:Item .

F2021L00304:170 a legcons:Item,
        owl:Class,
        dcat:Resource ;
    rdfs:label "Item - I170 8 23  Records of official marks manufactured or supplied"@en-AU ;
    dct:isPartOf F2021L00304:159 ;
    dct:isReferencedBy F2021L00304: ;
    rdfs:comment "8 23  Records of official marks manufactured or supplied - Abrievated Graph Key: I170"@en-AU ;
    skos:definition "8 23  Records of official marks manufactured or supplied"@en-AU ;
    skos:narrower F2021L00304:159 ;
    skos:prefLabel "Item I170"@en-AU ;
    dcat:accessURL <https://www.legislation.gov.au/F2021L00304/asmade/2021-03-24/text/original/epub/OEBPS/document_1/document_1.html#_Toc65844176> ;
    dcat:landingPage "https://www.legislation.gov.au/F2021L00304/asmade/2021-03-24/text/original/epub/OEBPS/document_1/document_1.html#_Toc65844176"^^xsd:anyURI ;
    dcat:theme legcons:Item .

F2021L00304:171 a legcons:Item,
        owl:Class,
        dcat:Resource ;
    rdfs:label "Item - I171 8 24  Records of official marks received applied removed defaced destroyed or returned"@en-AU ;
    dct:isPartOf F2021L00304:159 ;
    dct:isReferencedBy F2021L00304: ;
    rdfs:comment "8 24  Records of official marks received applied removed defaced destroyed or returned - Abrievated Graph Key: I171"@en-AU ;
    skos:definition "8 24  Records of official marks received applied removed defaced destroyed or returned"@en-AU ;
    skos:narrower F2021L00304:159 ;
    skos:prefLabel "Item I171"@en-AU ;
    dcat:accessURL <https://www.legislation.gov.au/F2021L00304/asmade/2021-03-24/text/original/epub/OEBPS/document_1/document_1.html#_Toc65844177> ;
    dcat:landingPage "https://www.legislation.gov.au/F2021L00304/asmade/2021-03-24/text/original/epub/OEBPS/document_1/document_1.html#_Toc65844177"^^xsd:anyURI ;
    dcat:theme legcons:Item .

F2021L00304:173 a legcons:Item,
        owl:Class,
        dcat:Resource ;
    rdfs:label "Item - I173 8 25  Purpose of this Division"@en-AU ;
    dct:isPartOf F2021L00304:172 ;
    dct:isReferencedBy F2021L00304: ;
    rdfs:comment "8 25  Purpose of this Division - Abrievated Graph Key: I173"@en-AU ;
    skos:definition "8 25  Purpose of this Division"@en-AU ;
    skos:narrower F2021L00304:172 ;
    skos:prefLabel "Item I173"@en-AU ;
    dcat:accessURL <https://www.legislation.gov.au/F2021L00304/asmade/2021-03-24/text/original/epub/OEBPS/document_1/document_1.html#_Toc65844179> ;
    dcat:landingPage "https://www.legislation.gov.au/F2021L00304/asmade/2021-03-24/text/original/epub/OEBPS/document_1/document_1.html#_Toc65844179"^^xsd:anyURI ;
    dcat:theme legcons:Item .

F2021L00304:174 a legcons:Item,
        owl:Class,
        dcat:Resource ;
    rdfs:label "Item - I174 8 26  Circumstances in which a mark resembles an official mark"@en-AU ;
    dct:isPartOf F2021L00304:172 ;
    dct:isReferencedBy F2021L00304: ;
    rdfs:comment "8 26  Circumstances in which a mark resembles an official mark - Abrievated Graph Key: I174"@en-AU ;
    skos:definition "8 26  Circumstances in which a mark resembles an official mark"@en-AU ;
    skos:narrower F2021L00304:172 ;
    skos:prefLabel "Item I174"@en-AU ;
    dcat:accessURL <https://www.legislation.gov.au/F2021L00304/asmade/2021-03-24/text/original/epub/OEBPS/document_1/document_1.html#_Toc65844180> ;
    dcat:landingPage "https://www.legislation.gov.au/F2021L00304/asmade/2021-03-24/text/original/epub/OEBPS/document_1/document_1.html#_Toc65844180"^^xsd:anyURI ;
    dcat:theme legcons:Item .

F2021L00304:175 a legcons:Item,
        owl:Class,
        dcat:Resource ;
    rdfs:label "Item - I175 8 27  Persons who may apply a resemblance"@en-AU ;
    dct:isPartOf F2021L00304:172 ;
    dct:isReferencedBy F2021L00304: ;
    rdfs:comment "8 27  Persons who may apply a resemblance - Abrievated Graph Key: I175"@en-AU ;
    skos:definition "8 27  Persons who may apply a resemblance"@en-AU ;
    skos:narrower F2021L00304:172 ;
    skos:prefLabel "Item I175"@en-AU ;
    dcat:accessURL <https://www.legislation.gov.au/F2021L00304/asmade/2021-03-24/text/original/epub/OEBPS/document_1/document_1.html#_Toc65844181> ;
    dcat:landingPage "https://www.legislation.gov.au/F2021L00304/asmade/2021-03-24/text/original/epub/OEBPS/document_1/document_1.html#_Toc65844181"^^xsd:anyURI ;
    dcat:theme legcons:Item .

F2021L00304:177 a legcons:Item,
        owl:Class,
        dcat:Resource ;
    rdfs:label "Item - I177 8 28  Purpose of this Division"@en-AU ;
    dct:isPartOf F2021L00304:176 ;
    dct:isReferencedBy F2021L00304: ;
    rdfs:comment "8 28  Purpose of this Division - Abrievated Graph Key: I177"@en-AU ;
    skos:definition "8 28  Purpose of this Division"@en-AU ;
    skos:narrower F2021L00304:176 ;
    skos:prefLabel "Item I177"@en-AU ;
    dcat:accessURL <https://www.legislation.gov.au/F2021L00304/asmade/2021-03-24/text/original/epub/OEBPS/document_1/document_1.html#_Toc65844183> ;
    dcat:landingPage "https://www.legislation.gov.au/F2021L00304/asmade/2021-03-24/text/original/epub/OEBPS/document_1/document_1.html#_Toc65844183"^^xsd:anyURI ;
    dcat:theme legcons:Item .

F2021L00304:178 a legcons:Item,
        owl:Class,
        dcat:Resource ;
    rdfs:label "Item - I178 8 29  Persons who may manufacture supply or possess official marking devices"@en-AU ;
    dct:isPartOf F2021L00304:176 ;
    dct:isReferencedBy F2021L00304: ;
    rdfs:comment "8 29  Persons who may manufacture supply or possess official marking devices - Abrievated Graph Key: I178"@en-AU ;
    skos:definition "8 29  Persons who may manufacture supply or possess official marking devices"@en-AU ;
    skos:narrower F2021L00304:176 ;
    skos:prefLabel "Item I178"@en-AU ;
    dcat:accessURL <https://www.legislation.gov.au/F2021L00304/asmade/2021-03-24/text/original/epub/OEBPS/document_1/document_1.html#_Toc65844184> ;
    dcat:landingPage "https://www.legislation.gov.au/F2021L00304/asmade/2021-03-24/text/original/epub/OEBPS/document_1/document_1.html#_Toc65844184"^^xsd:anyURI ;
    dcat:theme legcons:Item .

F2021L00304:179 a legcons:Item,
        owl:Class,
        dcat:Resource ;
    rdfs:label "Item - I179 8 30  Security of official marking devices"@en-AU ;
    dct:isPartOf F2021L00304:176 ;
    dct:isReferencedBy F2021L00304: ;
    rdfs:comment "8 30  Security of official marking devices - Abrievated Graph Key: I179"@en-AU ;
    skos:definition "8 30  Security of official marking devices"@en-AU ;
    skos:narrower F2021L00304:176 ;
    skos:prefLabel "Item I179"@en-AU ;
    dcat:accessURL <https://www.legislation.gov.au/F2021L00304/asmade/2021-03-24/text/original/epub/OEBPS/document_1/document_1.html#_Toc65844185> ;
    dcat:landingPage "https://www.legislation.gov.au/F2021L00304/asmade/2021-03-24/text/original/epub/OEBPS/document_1/document_1.html#_Toc65844185"^^xsd:anyURI ;
    dcat:theme legcons:Item .

F2021L00304:18 a legcons:Part,
        owl:Class,
        dcat:Resource ;
    rdfs:label "Part - P18 Part 2 Exemptions"@en-AU ;
    dct:isPartOf F2021L00304:10 ;
    dct:isReferencedBy F2021L00304: ;
    rdfs:comment "Part 2 Exemptions - Abrievated Graph Key: P18"@en-AU ;
    skos:definition "Part 2 Exemptions"@en-AU ;
    skos:narrower F2021L00304:10 ;
    skos:prefLabel "Part P18"@en-AU ;
    dcat:accessURL <https://www.legislation.gov.au/F2021L00304/asmade/2021-03-24/text/original/epub/OEBPS/document_1/document_1.html#_Toc65844024> ;
    dcat:landingPage "https://www.legislation.gov.au/F2021L00304/asmade/2021-03-24/text/original/epub/OEBPS/document_1/document_1.html#_Toc65844024"^^xsd:anyURI ;
    dcat:theme legcons:Part .

F2021L00304:180 a legcons:Item,
        owl:Class,
        dcat:Resource ;
    rdfs:label "Item - I180 8 31  Damaged etc official marking devices"@en-AU ;
    dct:isPartOf F2021L00304:176 ;
    dct:isReferencedBy F2021L00304: ;
    rdfs:comment "8 31  Damaged etc official marking devices - Abrievated Graph Key: I180"@en-AU ;
    skos:definition "8 31  Damaged etc official marking devices"@en-AU ;
    skos:narrower F2021L00304:176 ;
    skos:prefLabel "Item I180"@en-AU ;
    dcat:accessURL <https://www.legislation.gov.au/F2021L00304/asmade/2021-03-24/text/original/epub/OEBPS/document_1/document_1.html#_Toc65844186> ;
    dcat:landingPage "https://www.legislation.gov.au/F2021L00304/asmade/2021-03-24/text/original/epub/OEBPS/document_1/document_1.html#_Toc65844186"^^xsd:anyURI ;
    dcat:theme legcons:Item .

F2021L00304:181 a legcons:Item,
        owl:Class,
        dcat:Resource ;
    rdfs:label "Item - I181 8 32  Records of official marking devices manufactured or supplied"@en-AU ;
    dct:isPartOf F2021L00304:176 ;
    dct:isReferencedBy F2021L00304: ;
    rdfs:comment "8 32  Records of official marking devices manufactured or supplied - Abrievated Graph Key: I181"@en-AU ;
    skos:definition "8 32  Records of official marking devices manufactured or supplied"@en-AU ;
    skos:narrower F2021L00304:176 ;
    skos:prefLabel "Item I181"@en-AU ;
    dcat:accessURL <https://www.legislation.gov.au/F2021L00304/asmade/2021-03-24/text/original/epub/OEBPS/document_1/document_1.html#_Toc65844187> ;
    dcat:landingPage "https://www.legislation.gov.au/F2021L00304/asmade/2021-03-24/text/original/epub/OEBPS/document_1/document_1.html#_Toc65844187"^^xsd:anyURI ;
    dcat:theme legcons:Item .

F2021L00304:182 a legcons:Item,
        owl:Class,
        dcat:Resource ;
    rdfs:label "Item - I182 8 33  Records of official marking devices received used damaged destroyed or returned"@en-AU ;
    dct:isPartOf F2021L00304:176 ;
    dct:isReferencedBy F2021L00304: ;
    rdfs:comment "8 33  Records of official marking devices received used damaged destroyed or returned - Abrievated Graph Key: I182"@en-AU ;
    skos:definition "8 33  Records of official marking devices received used damaged destroyed or returned"@en-AU ;
    skos:narrower F2021L00304:176 ;
    skos:prefLabel "Item I182"@en-AU ;
    dcat:accessURL <https://www.legislation.gov.au/F2021L00304/asmade/2021-03-24/text/original/epub/OEBPS/document_1/document_1.html#_Toc65844188> ;
    dcat:landingPage "https://www.legislation.gov.au/F2021L00304/asmade/2021-03-24/text/original/epub/OEBPS/document_1/document_1.html#_Toc65844188"^^xsd:anyURI ;
    dcat:theme legcons:Item .

F2021L00304:186 a legcons:Item,
        owl:Class,
        dcat:Resource ;
    rdfs:label "Item - I186 9 1  References to audit in this Part"@en-AU ;
    dct:isPartOf F2021L00304:185 ;
    dct:isReferencedBy F2021L00304: ;
    rdfs:comment "9 1  References to audit in this Part - Abrievated Graph Key: I186"@en-AU ;
    skos:definition "9 1  References to audit in this Part"@en-AU ;
    skos:narrower F2021L00304:185 ;
    skos:prefLabel "Item I186"@en-AU ;
    dcat:accessURL <https://www.legislation.gov.au/F2021L00304/asmade/2021-03-24/text/original/epub/OEBPS/document_1/document_1.html#_Toc65844192> ;
    dcat:landingPage "https://www.legislation.gov.au/F2021L00304/asmade/2021-03-24/text/original/epub/OEBPS/document_1/document_1.html#_Toc65844192"^^xsd:anyURI ;
    dcat:theme legcons:Item .

F2021L00304:187 a legcons:Item,
        owl:Class,
        dcat:Resource ;
    rdfs:label "Item - I187 9 2  Audits of export operations"@en-AU ;
    dct:isPartOf F2021L00304:185 ;
    dct:isReferencedBy F2021L00304: ;
    rdfs:comment "9 2  Audits of export operations - Abrievated Graph Key: I187"@en-AU ;
    skos:definition "9 2  Audits of export operations"@en-AU ;
    skos:narrower F2021L00304:185 ;
    skos:prefLabel "Item I187"@en-AU ;
    dcat:accessURL <https://www.legislation.gov.au/F2021L00304/asmade/2021-03-24/text/original/epub/OEBPS/document_1/document_1.html#_Toc65844193> ;
    dcat:landingPage "https://www.legislation.gov.au/F2021L00304/asmade/2021-03-24/text/original/epub/OEBPS/document_1/document_1.html#_Toc65844193"^^xsd:anyURI ;
    dcat:theme legcons:Item .

F2021L00304:189 a legcons:Item,
        owl:Class,
        dcat:Resource ;
    rdfs:label "Item - I189 9 3  Purpose of this Division"@en-AU ;
    dct:isPartOf F2021L00304:188 ;
    dct:isReferencedBy F2021L00304: ;
    rdfs:comment "9 3  Purpose of this Division - Abrievated Graph Key: I189"@en-AU ;
    skos:definition "9 3  Purpose of this Division"@en-AU ;
    skos:narrower F2021L00304:188 ;
    skos:prefLabel "Item I189"@en-AU ;
    dcat:accessURL <https://www.legislation.gov.au/F2021L00304/asmade/2021-03-24/text/original/epub/OEBPS/document_1/document_1.html#_Toc65844195> ;
    dcat:landingPage "https://www.legislation.gov.au/F2021L00304/asmade/2021-03-24/text/original/epub/OEBPS/document_1/document_1.html#_Toc65844195"^^xsd:anyURI ;
    dcat:theme legcons:Item .

F2021L00304:19 a legcons:Item,
        owl:Class,
        dcat:Resource ;
    rdfs:label "Item - I19 2 5  Application of this Part"@en-AU ;
    dct:isPartOf F2021L00304:10 ;
    dct:isReferencedBy F2021L00304: ;
    rdfs:comment "2 5  Application of this Part - Abrievated Graph Key: I19"@en-AU ;
    skos:definition "2 5  Application of this Part"@en-AU ;
    skos:narrower F2021L00304:10 ;
    skos:prefLabel "Item I19"@en-AU ;
    dcat:accessURL <https://www.legislation.gov.au/F2021L00304/asmade/2021-03-24/text/original/epub/OEBPS/document_1/document_1.html#_Toc65844025> ;
    dcat:landingPage "https://www.legislation.gov.au/F2021L00304/asmade/2021-03-24/text/original/epub/OEBPS/document_1/document_1.html#_Toc65844025"^^xsd:anyURI ;
    dcat:theme legcons:Item .

F2021L00304:190 a legcons:Item,
        owl:Class,
        dcat:Resource ;
    rdfs:label "Item - I190 9 4  Manner in which audit must be conducted"@en-AU ;
    dct:isPartOf F2021L00304:188 ;
    dct:isReferencedBy F2021L00304: ;
    rdfs:comment "9 4  Manner in which audit must be conducted - Abrievated Graph Key: I190"@en-AU ;
    skos:definition "9 4  Manner in which audit must be conducted"@en-AU ;
    skos:narrower F2021L00304:188 ;
    skos:prefLabel "Item I190"@en-AU ;
    dcat:accessURL <https://www.legislation.gov.au/F2021L00304/asmade/2021-03-24/text/original/epub/OEBPS/document_1/document_1.html#_Toc65844196> ;
    dcat:landingPage "https://www.legislation.gov.au/F2021L00304/asmade/2021-03-24/text/original/epub/OEBPS/document_1/document_1.html#_Toc65844196"^^xsd:anyURI ;
    dcat:theme legcons:Item .

F2021L00304:191 a legcons:Item,
        owl:Class,
        dcat:Resource ;
    rdfs:label "Item - I191 9 5  Notice of non compliance with requirements"@en-AU ;
    dct:isPartOf F2021L00304:188 ;
    dct:isReferencedBy F2021L00304: ;
    rdfs:comment "9 5  Notice of non compliance with requirements - Abrievated Graph Key: I191"@en-AU ;
    skos:definition "9 5  Notice of non compliance with requirements"@en-AU ;
    skos:narrower F2021L00304:188 ;
    skos:prefLabel "Item I191"@en-AU ;
    dcat:accessURL <https://www.legislation.gov.au/F2021L00304/asmade/2021-03-24/text/original/epub/OEBPS/document_1/document_1.html#_Toc65844197> ;
    dcat:landingPage "https://www.legislation.gov.au/F2021L00304/asmade/2021-03-24/text/original/epub/OEBPS/document_1/document_1.html#_Toc65844197"^^xsd:anyURI ;
    dcat:theme legcons:Item .

F2021L00304:192 a legcons:Item,
        owl:Class,
        dcat:Resource ;
    rdfs:label "Item - I192 9 6  Audit reports"@en-AU ;
    dct:isPartOf F2021L00304:188 ;
    dct:isReferencedBy F2021L00304: ;
    rdfs:comment "9 6  Audit reports - Abrievated Graph Key: I192"@en-AU ;
    skos:definition "9 6  Audit reports"@en-AU ;
    skos:narrower F2021L00304:188 ;
    skos:prefLabel "Item I192"@en-AU ;
    dcat:accessURL <https://www.legislation.gov.au/F2021L00304/asmade/2021-03-24/text/original/epub/OEBPS/document_1/document_1.html#_Toc65844198> ;
    dcat:landingPage "https://www.legislation.gov.au/F2021L00304/asmade/2021-03-24/text/original/epub/OEBPS/document_1/document_1.html#_Toc65844198"^^xsd:anyURI ;
    dcat:theme legcons:Item .

F2021L00304:194 a legcons:Item,
        owl:Class,
        dcat:Resource ;
    rdfs:label "Item - I194 9 7  Purpose of this Division"@en-AU ;
    dct:isPartOf F2021L00304:193 ;
    dct:isReferencedBy F2021L00304: ;
    rdfs:comment "9 7  Purpose of this Division - Abrievated Graph Key: I194"@en-AU ;
    skos:definition "9 7  Purpose of this Division"@en-AU ;
    skos:narrower F2021L00304:193 ;
    skos:prefLabel "Item I194"@en-AU ;
    dcat:accessURL <https://www.legislation.gov.au/F2021L00304/asmade/2021-03-24/text/original/epub/OEBPS/document_1/document_1.html#_Toc65844200> ;
    dcat:landingPage "https://www.legislation.gov.au/F2021L00304/asmade/2021-03-24/text/original/epub/OEBPS/document_1/document_1.html#_Toc65844200"^^xsd:anyURI ;
    dcat:theme legcons:Item .

F2021L00304:195 a legcons:Item,
        owl:Class,
        dcat:Resource ;
    rdfs:label "Item - I195 9 8  Application for approval"@en-AU ;
    dct:isPartOf F2021L00304:193 ;
    dct:isReferencedBy F2021L00304: ;
    rdfs:comment "9 8  Application for approval - Abrievated Graph Key: I195"@en-AU ;
    skos:definition "9 8  Application for approval"@en-AU ;
    skos:narrower F2021L00304:193 ;
    skos:prefLabel "Item I195"@en-AU ;
    dcat:accessURL <https://www.legislation.gov.au/F2021L00304/asmade/2021-03-24/text/original/epub/OEBPS/document_1/document_1.html#_Toc65844201> ;
    dcat:landingPage "https://www.legislation.gov.au/F2021L00304/asmade/2021-03-24/text/original/epub/OEBPS/document_1/document_1.html#_Toc65844201"^^xsd:anyURI ;
    dcat:theme legcons:Item .

F2021L00304:196 a legcons:Item,
        owl:Class,
        dcat:Resource ;
    rdfs:label "Item - I196 9 9  Secretary must decide whether to approve applicant to conduct audits"@en-AU ;
    dct:isPartOf F2021L00304:193 ;
    dct:isReferencedBy F2021L00304: ;
    rdfs:comment "9 9  Secretary must decide whether to approve applicant to conduct audits - Abrievated Graph Key: I196"@en-AU ;
    skos:definition "9 9  Secretary must decide whether to approve applicant to conduct audits"@en-AU ;
    skos:narrower F2021L00304:193 ;
    skos:prefLabel "Item I196"@en-AU ;
    dcat:accessURL <https://www.legislation.gov.au/F2021L00304/asmade/2021-03-24/text/original/epub/OEBPS/document_1/document_1.html#_Toc65844202> ;
    dcat:landingPage "https://www.legislation.gov.au/F2021L00304/asmade/2021-03-24/text/original/epub/OEBPS/document_1/document_1.html#_Toc65844202"^^xsd:anyURI ;
    dcat:theme legcons:Item .

F2021L00304:197 a legcons:Item,
        owl:Class,
        dcat:Resource ;
    rdfs:label "Item - I197 9 10  Dealing with applications"@en-AU ;
    dct:isPartOf F2021L00304:193 ;
    dct:isReferencedBy F2021L00304: ;
    rdfs:comment "9 10  Dealing with applications - Abrievated Graph Key: I197"@en-AU ;
    skos:definition "9 10  Dealing with applications"@en-AU ;
    skos:narrower F2021L00304:193 ;
    skos:prefLabel "Item I197"@en-AU ;
    dcat:accessURL <https://www.legislation.gov.au/F2021L00304/asmade/2021-03-24/text/original/epub/OEBPS/document_1/document_1.html#_Toc65844203> ;
    dcat:landingPage "https://www.legislation.gov.au/F2021L00304/asmade/2021-03-24/text/original/epub/OEBPS/document_1/document_1.html#_Toc65844203"^^xsd:anyURI ;
    dcat:theme legcons:Item .

F2021L00304:198 a legcons:Item,
        owl:Class,
        dcat:Resource ;
    rdfs:label "Item - I198 9 11  Conditions of approval"@en-AU ;
    dct:isPartOf F2021L00304:193 ;
    dct:isReferencedBy F2021L00304: ;
    rdfs:comment "9 11  Conditions of approval - Abrievated Graph Key: I198"@en-AU ;
    skos:definition "9 11  Conditions of approval"@en-AU ;
    skos:narrower F2021L00304:193 ;
    skos:prefLabel "Item I198"@en-AU ;
    dcat:accessURL <https://www.legislation.gov.au/F2021L00304/asmade/2021-03-24/text/original/epub/OEBPS/document_1/document_1.html#_Toc65844204> ;
    dcat:landingPage "https://www.legislation.gov.au/F2021L00304/asmade/2021-03-24/text/original/epub/OEBPS/document_1/document_1.html#_Toc65844204"^^xsd:anyURI ;
    dcat:theme legcons:Item .

F2021L00304:199 a legcons:Item,
        owl:Class,
        dcat:Resource ;
    rdfs:label "Item - I199 9 12  Notice of decision"@en-AU ;
    dct:isPartOf F2021L00304:193 ;
    dct:isReferencedBy F2021L00304: ;
    rdfs:comment "9 12  Notice of decision - Abrievated Graph Key: I199"@en-AU ;
    skos:definition "9 12  Notice of decision"@en-AU ;
    skos:narrower F2021L00304:193 ;
    skos:prefLabel "Item I199"@en-AU ;
    dcat:accessURL <https://www.legislation.gov.au/F2021L00304/asmade/2021-03-24/text/original/epub/OEBPS/document_1/document_1.html#_Toc65844205> ;
    dcat:landingPage "https://www.legislation.gov.au/F2021L00304/asmade/2021-03-24/text/original/epub/OEBPS/document_1/document_1.html#_Toc65844205"^^xsd:anyURI ;
    dcat:theme legcons:Item .

F2021L00304:2 a legcons:Part,
        owl:Class,
        dcat:Resource ;
    rdfs:label "Part - P2 Part 1 Preliminary"@en-AU ;
    dct:isPartOf F2021L00304:1 ;
    dct:isReferencedBy F2021L00304: ;
    rdfs:comment "Part 1 Preliminary - Abrievated Graph Key: P2"@en-AU ;
    skos:definition "Part 1 Preliminary"@en-AU ;
    skos:narrower F2021L00304:1 ;
    skos:prefLabel "Part P2"@en-AU ;
    dcat:accessURL <https://www.legislation.gov.au/F2021L00304/asmade/2021-03-24/text/original/epub/OEBPS/document_1/document_1.html#_Toc65844008> ;
    dcat:landingPage "https://www.legislation.gov.au/F2021L00304/asmade/2021-03-24/text/original/epub/OEBPS/document_1/document_1.html#_Toc65844008"^^xsd:anyURI ;
    dcat:theme legcons:Part .

F2021L00304:20 a legcons:Item,
        owl:Class,
        dcat:Resource ;
    rdfs:label "Item - I20 2 6  Prescribed circumstancetesting the market"@en-AU ;
    dct:isPartOf F2021L00304:10 ;
    dct:isReferencedBy F2021L00304: ;
    rdfs:comment "2 6  Prescribed circumstancetesting the market - Abrievated Graph Key: I20"@en-AU ;
    skos:definition "2 6  Prescribed circumstancetesting the market"@en-AU ;
    skos:narrower F2021L00304:10 ;
    skos:prefLabel "Item I20"@en-AU ;
    dcat:accessURL <https://www.legislation.gov.au/F2021L00304/asmade/2021-03-24/text/original/epub/OEBPS/document_1/document_1.html#_Toc65844026> ;
    dcat:landingPage "https://www.legislation.gov.au/F2021L00304/asmade/2021-03-24/text/original/epub/OEBPS/document_1/document_1.html#_Toc65844026"^^xsd:anyURI ;
    dcat:theme legcons:Item .

F2021L00304:200 a legcons:Item,
        owl:Class,
        dcat:Resource ;
    rdfs:label "Item - I200 9 13  Period of effect of approval"@en-AU ;
    dct:isPartOf F2021L00304:193 ;
    dct:isReferencedBy F2021L00304: ;
    rdfs:comment "9 13  Period of effect of approval - Abrievated Graph Key: I200"@en-AU ;
    skos:definition "9 13  Period of effect of approval"@en-AU ;
    skos:narrower F2021L00304:193 ;
    skos:prefLabel "Item I200"@en-AU ;
    dcat:accessURL <https://www.legislation.gov.au/F2021L00304/asmade/2021-03-24/text/original/epub/OEBPS/document_1/document_1.html#_Toc65844206> ;
    dcat:landingPage "https://www.legislation.gov.au/F2021L00304/asmade/2021-03-24/text/original/epub/OEBPS/document_1/document_1.html#_Toc65844206"^^xsd:anyURI ;
    dcat:theme legcons:Item .

F2021L00304:201 a legcons:Item,
        owl:Class,
        dcat:Resource ;
    rdfs:label "Item - I201 9 14  Imposing or varying conditions of approval"@en-AU ;
    dct:isPartOf F2021L00304:193 ;
    dct:isReferencedBy F2021L00304: ;
    rdfs:comment "9 14  Imposing or varying conditions of approval - Abrievated Graph Key: I201"@en-AU ;
    skos:definition "9 14  Imposing or varying conditions of approval"@en-AU ;
    skos:narrower F2021L00304:193 ;
    skos:prefLabel "Item I201"@en-AU ;
    dcat:accessURL <https://www.legislation.gov.au/F2021L00304/asmade/2021-03-24/text/original/epub/OEBPS/document_1/document_1.html#_Toc65844207> ;
    dcat:landingPage "https://www.legislation.gov.au/F2021L00304/asmade/2021-03-24/text/original/epub/OEBPS/document_1/document_1.html#_Toc65844207"^^xsd:anyURI ;
    dcat:theme legcons:Item .

F2021L00304:202 a legcons:Item,
        owl:Class,
        dcat:Resource ;
    rdfs:label "Item - I202 9 15  Revocation of approval"@en-AU ;
    dct:isPartOf F2021L00304:193 ;
    dct:isReferencedBy F2021L00304: ;
    rdfs:comment "9 15  Revocation of approval - Abrievated Graph Key: I202"@en-AU ;
    skos:definition "9 15  Revocation of approval"@en-AU ;
    skos:narrower F2021L00304:193 ;
    skos:prefLabel "Item I202"@en-AU ;
    dcat:accessURL <https://www.legislation.gov.au/F2021L00304/asmade/2021-03-24/text/original/epub/OEBPS/document_1/document_1.html#_Toc65844208> ;
    dcat:landingPage "https://www.legislation.gov.au/F2021L00304/asmade/2021-03-24/text/original/epub/OEBPS/document_1/document_1.html#_Toc65844208"^^xsd:anyURI ;
    dcat:theme legcons:Item .

F2021L00304:203 a legcons:Item,
        owl:Class,
        dcat:Resource ;
    rdfs:label "Item - I203 9 16  Register of approved auditors"@en-AU ;
    dct:isPartOf F2021L00304:193 ;
    dct:isReferencedBy F2021L00304: ;
    rdfs:comment "9 16  Register of approved auditors - Abrievated Graph Key: I203"@en-AU ;
    skos:definition "9 16  Register of approved auditors"@en-AU ;
    skos:narrower F2021L00304:193 ;
    skos:prefLabel "Item I203"@en-AU ;
    dcat:accessURL <https://www.legislation.gov.au/F2021L00304/asmade/2021-03-24/text/original/epub/OEBPS/document_1/document_1.html#_Toc65844209> ;
    dcat:landingPage "https://www.legislation.gov.au/F2021L00304/asmade/2021-03-24/text/original/epub/OEBPS/document_1/document_1.html#_Toc65844209"^^xsd:anyURI ;
    dcat:theme legcons:Item .

F2021L00304:204 a legcons:Item,
        owl:Class,
        dcat:Resource ;
    rdfs:label "Item - I204 9 17  Fit and proper person test"@en-AU ;
    dct:isPartOf F2021L00304:193 ;
    dct:isReferencedBy F2021L00304: ;
    rdfs:comment "9 17  Fit and proper person test - Abrievated Graph Key: I204"@en-AU ;
    skos:definition "9 17  Fit and proper person test"@en-AU ;
    skos:narrower F2021L00304:193 ;
    skos:prefLabel "Item I204"@en-AU ;
    dcat:accessURL <https://www.legislation.gov.au/F2021L00304/asmade/2021-03-24/text/original/epub/OEBPS/document_1/document_1.html#_Toc65844210> ;
    dcat:landingPage "https://www.legislation.gov.au/F2021L00304/asmade/2021-03-24/text/original/epub/OEBPS/document_1/document_1.html#_Toc65844210"^^xsd:anyURI ;
    dcat:theme legcons:Item .

F2021L00304:207 a legcons:Item,
        owl:Class,
        dcat:Resource ;
    rdfs:label "Item - I207 9 18  References to assessment in this Part"@en-AU ;
    dct:isPartOf F2021L00304:206 ;
    dct:isReferencedBy F2021L00304: ;
    rdfs:comment "9 18  References to assessment in this Part - Abrievated Graph Key: I207"@en-AU ;
    skos:definition "9 18  References to assessment in this Part"@en-AU ;
    skos:narrower F2021L00304:206 ;
    skos:prefLabel "Item I207"@en-AU ;
    dcat:accessURL <https://www.legislation.gov.au/F2021L00304/asmade/2021-03-24/text/original/epub/OEBPS/document_1/document_1.html#_Toc65844213> ;
    dcat:landingPage "https://www.legislation.gov.au/F2021L00304/asmade/2021-03-24/text/original/epub/OEBPS/document_1/document_1.html#_Toc65844213"^^xsd:anyURI ;
    dcat:theme legcons:Item .

F2021L00304:209 a legcons:Item,
        owl:Class,
        dcat:Resource ;
    rdfs:label "Item - I209 9 19  Circumstances in which assessment may be required or permitted"@en-AU ;
    dct:isPartOf F2021L00304:208 ;
    dct:isReferencedBy F2021L00304: ;
    rdfs:comment "9 19  Circumstances in which assessment may be required or permitted - Abrievated Graph Key: I209"@en-AU ;
    skos:definition "9 19  Circumstances in which assessment may be required or permitted"@en-AU ;
    skos:narrower F2021L00304:208 ;
    skos:prefLabel "Item I209"@en-AU ;
    dcat:accessURL <https://www.legislation.gov.au/F2021L00304/asmade/2021-03-24/text/original/epub/OEBPS/document_1/document_1.html#_Toc65844215> ;
    dcat:landingPage "https://www.legislation.gov.au/F2021L00304/asmade/2021-03-24/text/original/epub/OEBPS/document_1/document_1.html#_Toc65844215"^^xsd:anyURI ;
    dcat:theme legcons:Item .

F2021L00304:21 a legcons:Item,
        owl:Class,
        dcat:Resource ;
    rdfs:label "Item - I21 2 7  Prescribed meaningcommercial sample"@en-AU ;
    dct:isPartOf F2021L00304:10 ;
    dct:isReferencedBy F2021L00304: ;
    rdfs:comment "2 7  Prescribed meaningcommercial sample - Abrievated Graph Key: I21"@en-AU ;
    skos:definition "2 7  Prescribed meaningcommercial sample"@en-AU ;
    skos:narrower F2021L00304:10 ;
    skos:prefLabel "Item I21"@en-AU ;
    dcat:accessURL <https://www.legislation.gov.au/F2021L00304/asmade/2021-03-24/text/original/epub/OEBPS/document_1/document_1.html#_Toc65844027> ;
    dcat:landingPage "https://www.legislation.gov.au/F2021L00304/asmade/2021-03-24/text/original/epub/OEBPS/document_1/document_1.html#_Toc65844027"^^xsd:anyURI ;
    dcat:theme legcons:Item .

F2021L00304:210 a legcons:Item,
        owl:Class,
        dcat:Resource ;
    rdfs:label "Item - I210 9 20  Process to be followed after assessment completed"@en-AU ;
    dct:isPartOf F2021L00304:208 ;
    dct:isReferencedBy F2021L00304: ;
    rdfs:comment "9 20  Process to be followed after assessment completed - Abrievated Graph Key: I210"@en-AU ;
    skos:definition "9 20  Process to be followed after assessment completed"@en-AU ;
    skos:narrower F2021L00304:208 ;
    skos:prefLabel "Item I210"@en-AU ;
    dcat:accessURL <https://www.legislation.gov.au/F2021L00304/asmade/2021-03-24/text/original/epub/OEBPS/document_1/document_1.html#_Toc65844216> ;
    dcat:landingPage "https://www.legislation.gov.au/F2021L00304/asmade/2021-03-24/text/original/epub/OEBPS/document_1/document_1.html#_Toc65844216"^^xsd:anyURI ;
    dcat:theme legcons:Item .

F2021L00304:212 a legcons:Item,
        owl:Class,
        dcat:Resource ;
    rdfs:label "Item - I212 9 21  Purpose of this Division"@en-AU ;
    dct:isPartOf F2021L00304:211 ;
    dct:isReferencedBy F2021L00304: ;
    rdfs:comment "9 21  Purpose of this Division - Abrievated Graph Key: I212"@en-AU ;
    skos:definition "9 21  Purpose of this Division"@en-AU ;
    skos:narrower F2021L00304:211 ;
    skos:prefLabel "Item I212"@en-AU ;
    dcat:accessURL <https://www.legislation.gov.au/F2021L00304/asmade/2021-03-24/text/original/epub/OEBPS/document_1/document_1.html#_Toc65844218> ;
    dcat:landingPage "https://www.legislation.gov.au/F2021L00304/asmade/2021-03-24/text/original/epub/OEBPS/document_1/document_1.html#_Toc65844218"^^xsd:anyURI ;
    dcat:theme legcons:Item .

F2021L00304:213 a legcons:Item,
        owl:Class,
        dcat:Resource ;
    rdfs:label "Item - I213 9 22  Application for approval"@en-AU ;
    dct:isPartOf F2021L00304:211 ;
    dct:isReferencedBy F2021L00304: ;
    rdfs:comment "9 22  Application for approval - Abrievated Graph Key: I213"@en-AU ;
    skos:definition "9 22  Application for approval"@en-AU ;
    skos:narrower F2021L00304:211 ;
    skos:prefLabel "Item I213"@en-AU ;
    dcat:accessURL <https://www.legislation.gov.au/F2021L00304/asmade/2021-03-24/text/original/epub/OEBPS/document_1/document_1.html#_Toc65844219> ;
    dcat:landingPage "https://www.legislation.gov.au/F2021L00304/asmade/2021-03-24/text/original/epub/OEBPS/document_1/document_1.html#_Toc65844219"^^xsd:anyURI ;
    dcat:theme legcons:Item .

F2021L00304:214 a legcons:Item,
        owl:Class,
        dcat:Resource ;
    rdfs:label "Item - I214 9 23  Secretary must decide whether to approve applicant to carry out assessments"@en-AU ;
    dct:isPartOf F2021L00304:211 ;
    dct:isReferencedBy F2021L00304: ;
    rdfs:comment "9 23  Secretary must decide whether to approve applicant to carry out assessments - Abrievated Graph Key: I214"@en-AU ;
    skos:definition "9 23  Secretary must decide whether to approve applicant to carry out assessments"@en-AU ;
    skos:narrower F2021L00304:211 ;
    skos:prefLabel "Item I214"@en-AU ;
    dcat:accessURL <https://www.legislation.gov.au/F2021L00304/asmade/2021-03-24/text/original/epub/OEBPS/document_1/document_1.html#_Toc65844220> ;
    dcat:landingPage "https://www.legislation.gov.au/F2021L00304/asmade/2021-03-24/text/original/epub/OEBPS/document_1/document_1.html#_Toc65844220"^^xsd:anyURI ;
    dcat:theme legcons:Item .

F2021L00304:215 a legcons:Item,
        owl:Class,
        dcat:Resource ;
    rdfs:label "Item - I215 9 24  Dealing with applications"@en-AU ;
    dct:isPartOf F2021L00304:211 ;
    dct:isReferencedBy F2021L00304: ;
    rdfs:comment "9 24  Dealing with applications - Abrievated Graph Key: I215"@en-AU ;
    skos:definition "9 24  Dealing with applications"@en-AU ;
    skos:narrower F2021L00304:211 ;
    skos:prefLabel "Item I215"@en-AU ;
    dcat:accessURL <https://www.legislation.gov.au/F2021L00304/asmade/2021-03-24/text/original/epub/OEBPS/document_1/document_1.html#_Toc65844221> ;
    dcat:landingPage "https://www.legislation.gov.au/F2021L00304/asmade/2021-03-24/text/original/epub/OEBPS/document_1/document_1.html#_Toc65844221"^^xsd:anyURI ;
    dcat:theme legcons:Item .

F2021L00304:216 a legcons:Item,
        owl:Class,
        dcat:Resource ;
    rdfs:label "Item - I216 9 25  Conditions of approval"@en-AU ;
    dct:isPartOf F2021L00304:211 ;
    dct:isReferencedBy F2021L00304: ;
    rdfs:comment "9 25  Conditions of approval - Abrievated Graph Key: I216"@en-AU ;
    skos:definition "9 25  Conditions of approval"@en-AU ;
    skos:narrower F2021L00304:211 ;
    skos:prefLabel "Item I216"@en-AU ;
    dcat:accessURL <https://www.legislation.gov.au/F2021L00304/asmade/2021-03-24/text/original/epub/OEBPS/document_1/document_1.html#_Toc65844222> ;
    dcat:landingPage "https://www.legislation.gov.au/F2021L00304/asmade/2021-03-24/text/original/epub/OEBPS/document_1/document_1.html#_Toc65844222"^^xsd:anyURI ;
    dcat:theme legcons:Item .

F2021L00304:217 a legcons:Item,
        owl:Class,
        dcat:Resource ;
    rdfs:label "Item - I217 9 26  Notice of decision"@en-AU ;
    dct:isPartOf F2021L00304:211 ;
    dct:isReferencedBy F2021L00304: ;
    rdfs:comment "9 26  Notice of decision - Abrievated Graph Key: I217"@en-AU ;
    skos:definition "9 26  Notice of decision"@en-AU ;
    skos:narrower F2021L00304:211 ;
    skos:prefLabel "Item I217"@en-AU ;
    dcat:accessURL <https://www.legislation.gov.au/F2021L00304/asmade/2021-03-24/text/original/epub/OEBPS/document_1/document_1.html#_Toc65844223> ;
    dcat:landingPage "https://www.legislation.gov.au/F2021L00304/asmade/2021-03-24/text/original/epub/OEBPS/document_1/document_1.html#_Toc65844223"^^xsd:anyURI ;
    dcat:theme legcons:Item .

F2021L00304:218 a legcons:Item,
        owl:Class,
        dcat:Resource ;
    rdfs:label "Item - I218 9 27  Period of effect of approval"@en-AU ;
    dct:isPartOf F2021L00304:211 ;
    dct:isReferencedBy F2021L00304: ;
    rdfs:comment "9 27  Period of effect of approval - Abrievated Graph Key: I218"@en-AU ;
    skos:definition "9 27  Period of effect of approval"@en-AU ;
    skos:narrower F2021L00304:211 ;
    skos:prefLabel "Item I218"@en-AU ;
    dcat:accessURL <https://www.legislation.gov.au/F2021L00304/asmade/2021-03-24/text/original/epub/OEBPS/document_1/document_1.html#_Toc65844224> ;
    dcat:landingPage "https://www.legislation.gov.au/F2021L00304/asmade/2021-03-24/text/original/epub/OEBPS/document_1/document_1.html#_Toc65844224"^^xsd:anyURI ;
    dcat:theme legcons:Item .

F2021L00304:219 a legcons:Item,
        owl:Class,
        dcat:Resource ;
    rdfs:label "Item - I219 9 28  Imposing or varying conditions of approval"@en-AU ;
    dct:isPartOf F2021L00304:211 ;
    dct:isReferencedBy F2021L00304: ;
    rdfs:comment "9 28  Imposing or varying conditions of approval - Abrievated Graph Key: I219"@en-AU ;
    skos:definition "9 28  Imposing or varying conditions of approval"@en-AU ;
    skos:narrower F2021L00304:211 ;
    skos:prefLabel "Item I219"@en-AU ;
    dcat:accessURL <https://www.legislation.gov.au/F2021L00304/asmade/2021-03-24/text/original/epub/OEBPS/document_1/document_1.html#_Toc65844225> ;
    dcat:landingPage "https://www.legislation.gov.au/F2021L00304/asmade/2021-03-24/text/original/epub/OEBPS/document_1/document_1.html#_Toc65844225"^^xsd:anyURI ;
    dcat:theme legcons:Item .

F2021L00304:22 a legcons:Item,
        owl:Class,
        dcat:Resource ;
    rdfs:label "Item - I22 2 8  Period for making application for exemption"@en-AU ;
    dct:isPartOf F2021L00304:10 ;
    dct:isReferencedBy F2021L00304: ;
    rdfs:comment "2 8  Period for making application for exemption - Abrievated Graph Key: I22"@en-AU ;
    skos:definition "2 8  Period for making application for exemption"@en-AU ;
    skos:narrower F2021L00304:10 ;
    skos:prefLabel "Item I22"@en-AU ;
    dcat:accessURL <https://www.legislation.gov.au/F2021L00304/asmade/2021-03-24/text/original/epub/OEBPS/document_1/document_1.html#_Toc65844028> ;
    dcat:landingPage "https://www.legislation.gov.au/F2021L00304/asmade/2021-03-24/text/original/epub/OEBPS/document_1/document_1.html#_Toc65844028"^^xsd:anyURI ;
    dcat:theme legcons:Item .

F2021L00304:220 a legcons:Item,
        owl:Class,
        dcat:Resource ;
    rdfs:label "Item - I220 9 29  Revocation of approval"@en-AU ;
    dct:isPartOf F2021L00304:211 ;
    dct:isReferencedBy F2021L00304: ;
    rdfs:comment "9 29  Revocation of approval - Abrievated Graph Key: I220"@en-AU ;
    skos:definition "9 29  Revocation of approval"@en-AU ;
    skos:narrower F2021L00304:211 ;
    skos:prefLabel "Item I220"@en-AU ;
    dcat:accessURL <https://www.legislation.gov.au/F2021L00304/asmade/2021-03-24/text/original/epub/OEBPS/document_1/document_1.html#_Toc65844226> ;
    dcat:landingPage "https://www.legislation.gov.au/F2021L00304/asmade/2021-03-24/text/original/epub/OEBPS/document_1/document_1.html#_Toc65844226"^^xsd:anyURI ;
    dcat:theme legcons:Item .

F2021L00304:221 a legcons:Item,
        owl:Class,
        dcat:Resource ;
    rdfs:label "Item - I221 9 30  Register of approved assessors"@en-AU ;
    dct:isPartOf F2021L00304:211 ;
    dct:isReferencedBy F2021L00304: ;
    rdfs:comment "9 30  Register of approved assessors - Abrievated Graph Key: I221"@en-AU ;
    skos:definition "9 30  Register of approved assessors"@en-AU ;
    skos:narrower F2021L00304:211 ;
    skos:prefLabel "Item I221"@en-AU ;
    dcat:accessURL <https://www.legislation.gov.au/F2021L00304/asmade/2021-03-24/text/original/epub/OEBPS/document_1/document_1.html#_Toc65844227> ;
    dcat:landingPage "https://www.legislation.gov.au/F2021L00304/asmade/2021-03-24/text/original/epub/OEBPS/document_1/document_1.html#_Toc65844227"^^xsd:anyURI ;
    dcat:theme legcons:Item .

F2021L00304:222 a legcons:Item,
        owl:Class,
        dcat:Resource ;
    rdfs:label "Item - I222 9 31  Fit and proper person test"@en-AU ;
    dct:isPartOf F2021L00304:211 ;
    dct:isReferencedBy F2021L00304: ;
    rdfs:comment "9 31  Fit and proper person test - Abrievated Graph Key: I222"@en-AU ;
    skos:definition "9 31  Fit and proper person test"@en-AU ;
    skos:narrower F2021L00304:211 ;
    skos:prefLabel "Item I222"@en-AU ;
    dcat:accessURL <https://www.legislation.gov.au/F2021L00304/asmade/2021-03-24/text/original/epub/OEBPS/document_1/document_1.html#_Toc65844228> ;
    dcat:landingPage "https://www.legislation.gov.au/F2021L00304/asmade/2021-03-24/text/original/epub/OEBPS/document_1/document_1.html#_Toc65844228"^^xsd:anyURI ;
    dcat:theme legcons:Item .

F2021L00304:224 a legcons:Item,
        owl:Class,
        dcat:Resource ;
    rdfs:label "Item - I224 9 32  Decisions that may be made by operation of computer program"@en-AU ;
    dct:isPartOf F2021L00304:223 ;
    dct:isReferencedBy F2021L00304: ;
    rdfs:comment "9 32  Decisions that may be made by operation of computer program - Abrievated Graph Key: I224"@en-AU ;
    skos:definition "9 32  Decisions that may be made by operation of computer program"@en-AU ;
    skos:narrower F2021L00304:223 ;
    skos:prefLabel "Item I224"@en-AU ;
    dcat:accessURL <https://www.legislation.gov.au/F2021L00304/asmade/2021-03-24/text/original/epub/OEBPS/document_1/document_1.html#_Toc65844230> ;
    dcat:landingPage "https://www.legislation.gov.au/F2021L00304/asmade/2021-03-24/text/original/epub/OEBPS/document_1/document_1.html#_Toc65844230"^^xsd:anyURI ;
    dcat:theme legcons:Item .

F2021L00304:227 a legcons:Item,
        owl:Class,
        dcat:Resource ;
    rdfs:label "Item - I227 9 33  Requirement to be third party authorised officerfit and proper person etc"@en-AU ;
    dct:isPartOf F2021L00304:226 ;
    dct:isReferencedBy F2021L00304: ;
    rdfs:comment "9 33  Requirement to be third party authorised officerfit and proper person etc - Abrievated Graph Key: I227"@en-AU ;
    skos:definition "9 33  Requirement to be third party authorised officerfit and proper person etc"@en-AU ;
    skos:narrower F2021L00304:226 ;
    skos:prefLabel "Item I227"@en-AU ;
    dcat:accessURL <https://www.legislation.gov.au/F2021L00304/asmade/2021-03-24/text/original/epub/OEBPS/document_1/document_1.html#_Toc65844233> ;
    dcat:landingPage "https://www.legislation.gov.au/F2021L00304/asmade/2021-03-24/text/original/epub/OEBPS/document_1/document_1.html#_Toc65844233"^^xsd:anyURI ;
    dcat:theme legcons:Item .

F2021L00304:229 a legcons:Item,
        owl:Class,
        dcat:Resource ;
    rdfs:label "Item - I229 9 34  Purpose of this Division"@en-AU ;
    dct:isPartOf F2021L00304:228 ;
    dct:isReferencedBy F2021L00304: ;
    rdfs:comment "9 34  Purpose of this Division - Abrievated Graph Key: I229"@en-AU ;
    skos:definition "9 34  Purpose of this Division"@en-AU ;
    skos:narrower F2021L00304:228 ;
    skos:prefLabel "Item I229"@en-AU ;
    dcat:accessURL <https://www.legislation.gov.au/F2021L00304/asmade/2021-03-24/text/original/epub/OEBPS/document_1/document_1.html#_Toc65844235> ;
    dcat:landingPage "https://www.legislation.gov.au/F2021L00304/asmade/2021-03-24/text/original/epub/OEBPS/document_1/document_1.html#_Toc65844235"^^xsd:anyURI ;
    dcat:theme legcons:Item .

F2021L00304:23 a legcons:Item,
        owl:Class,
        dcat:Resource ;
    rdfs:label "Item - I23 2 9  Conditions of exemptionmatters to which Secretary must have regard"@en-AU ;
    dct:isPartOf F2021L00304:10 ;
    dct:isReferencedBy F2021L00304: ;
    rdfs:comment "2 9  Conditions of exemptionmatters to which Secretary must have regard - Abrievated Graph Key: I23"@en-AU ;
    skos:definition "2 9  Conditions of exemptionmatters to which Secretary must have regard"@en-AU ;
    skos:narrower F2021L00304:10 ;
    skos:prefLabel "Item I23"@en-AU ;
    dcat:accessURL <https://www.legislation.gov.au/F2021L00304/asmade/2021-03-24/text/original/epub/OEBPS/document_1/document_1.html#_Toc65844029> ;
    dcat:landingPage "https://www.legislation.gov.au/F2021L00304/asmade/2021-03-24/text/original/epub/OEBPS/document_1/document_1.html#_Toc65844029"^^xsd:anyURI ;
    dcat:theme legcons:Item .

F2021L00304:230 a legcons:Item,
        owl:Class,
        dcat:Resource ;
    rdfs:label "Item - I230 9 35  Inspecting establishments and securing areas facilities equipment or other things"@en-AU ;
    dct:isPartOf F2021L00304:228 ;
    dct:isReferencedBy F2021L00304: ;
    rdfs:comment "9 35  Inspecting establishments and securing areas facilities equipment or other things - Abrievated Graph Key: I230"@en-AU ;
    skos:definition "9 35  Inspecting establishments and securing areas facilities equipment or other things"@en-AU ;
    skos:narrower F2021L00304:228 ;
    skos:prefLabel "Item I230"@en-AU ;
    dcat:accessURL <https://www.legislation.gov.au/F2021L00304/asmade/2021-03-24/text/original/epub/OEBPS/document_1/document_1.html#_Toc65844236> ;
    dcat:landingPage "https://www.legislation.gov.au/F2021L00304/asmade/2021-03-24/text/original/epub/OEBPS/document_1/document_1.html#_Toc65844236"^^xsd:anyURI ;
    dcat:theme legcons:Item .

F2021L00304:231 a legcons:Item,
        owl:Class,
        dcat:Resource ;
    rdfs:label "Item - I231 9 36  Securing and identifying establishment or conveyance etc"@en-AU ;
    dct:isPartOf F2021L00304:228 ;
    dct:isReferencedBy F2021L00304: ;
    rdfs:comment "9 36  Securing and identifying establishment or conveyance etc - Abrievated Graph Key: I231"@en-AU ;
    skos:definition "9 36  Securing and identifying establishment or conveyance etc"@en-AU ;
    skos:narrower F2021L00304:228 ;
    skos:prefLabel "Item I231"@en-AU ;
    dcat:accessURL <https://www.legislation.gov.au/F2021L00304/asmade/2021-03-24/text/original/epub/OEBPS/document_1/document_1.html#_Toc65844237> ;
    dcat:landingPage "https://www.legislation.gov.au/F2021L00304/asmade/2021-03-24/text/original/epub/OEBPS/document_1/document_1.html#_Toc65844237"^^xsd:anyURI ;
    dcat:theme legcons:Item .

F2021L00304:232 a legcons:Item,
        owl:Class,
        dcat:Resource ;
    rdfs:label "Item - I232 9 37  Interference with identified establishment or conveyance etc"@en-AU ;
    dct:isPartOf F2021L00304:228 ;
    dct:isReferencedBy F2021L00304: ;
    rdfs:comment "9 37  Interference with identified establishment or conveyance etc - Abrievated Graph Key: I232"@en-AU ;
    skos:definition "9 37  Interference with identified establishment or conveyance etc"@en-AU ;
    skos:narrower F2021L00304:228 ;
    skos:prefLabel "Item I232"@en-AU ;
    dcat:accessURL <https://www.legislation.gov.au/F2021L00304/asmade/2021-03-24/text/original/epub/OEBPS/document_1/document_1.html#_Toc65844238> ;
    dcat:landingPage "https://www.legislation.gov.au/F2021L00304/asmade/2021-03-24/text/original/epub/OEBPS/document_1/document_1.html#_Toc65844238"^^xsd:anyURI ;
    dcat:theme legcons:Item .

F2021L00304:234 a legcons:Item,
        owl:Class,
        dcat:Resource ;
    rdfs:label "Item - I234 9 38  Other grounds for giving direction"@en-AU ;
    dct:isPartOf F2021L00304:233 ;
    dct:isReferencedBy F2021L00304: ;
    rdfs:comment "9 38  Other grounds for giving direction - Abrievated Graph Key: I234"@en-AU ;
    skos:definition "9 38  Other grounds for giving direction"@en-AU ;
    skos:narrower F2021L00304:233 ;
    skos:prefLabel "Item I234"@en-AU ;
    dcat:accessURL <https://www.legislation.gov.au/F2021L00304/asmade/2021-03-24/text/original/epub/OEBPS/document_1/document_1.html#_Toc65844240> ;
    dcat:landingPage "https://www.legislation.gov.au/F2021L00304/asmade/2021-03-24/text/original/epub/OEBPS/document_1/document_1.html#_Toc65844240"^^xsd:anyURI ;
    dcat:theme legcons:Item .

F2021L00304:236 a legcons:Item,
        owl:Class,
        dcat:Resource ;
    rdfs:label "Item - I236 9 39  Circumstances in which identity card need not be carried"@en-AU ;
    dct:isPartOf F2021L00304:235 ;
    dct:isReferencedBy F2021L00304: ;
    rdfs:comment "9 39  Circumstances in which identity card need not be carried - Abrievated Graph Key: I236"@en-AU ;
    skos:definition "9 39  Circumstances in which identity card need not be carried"@en-AU ;
    skos:narrower F2021L00304:235 ;
    skos:prefLabel "Item I236"@en-AU ;
    dcat:accessURL <https://www.legislation.gov.au/F2021L00304/asmade/2021-03-24/text/original/epub/OEBPS/document_1/document_1.html#_Toc65844242> ;
    dcat:landingPage "https://www.legislation.gov.au/F2021L00304/asmade/2021-03-24/text/original/epub/OEBPS/document_1/document_1.html#_Toc65844242"^^xsd:anyURI ;
    dcat:theme legcons:Item .

F2021L00304:238 a legcons:Item,
        owl:Class,
        dcat:Resource ;
    rdfs:label "Item - I238 10 1  Samples taken in exercising monitoring or investigation powers"@en-AU ;
    dct:isPartOf F2021L00304:237 ;
    dct:isReferencedBy F2021L00304: ;
    rdfs:comment "10 1  Samples taken in exercising monitoring or investigation powers - Abrievated Graph Key: I238"@en-AU ;
    skos:definition "10 1  Samples taken in exercising monitoring or investigation powers"@en-AU ;
    skos:narrower F2021L00304:237 ;
    skos:prefLabel "Item I238"@en-AU ;
    dcat:accessURL <https://www.legislation.gov.au/F2021L00304/asmade/2021-03-24/text/original/epub/OEBPS/document_1/document_1.html#_Toc65844244> ;
    dcat:landingPage "https://www.legislation.gov.au/F2021L00304/asmade/2021-03-24/text/original/epub/OEBPS/document_1/document_1.html#_Toc65844244"^^xsd:anyURI ;
    dcat:theme legcons:Item .

F2021L00304:239 a legcons:Item,
        owl:Class,
        dcat:Resource ;
    rdfs:label "Item - I239 10 2  Dealing with things seized in exercising investigation powers"@en-AU ;
    dct:isPartOf F2021L00304:237 ;
    dct:isReferencedBy F2021L00304: ;
    rdfs:comment "10 2  Dealing with things seized in exercising investigation powers - Abrievated Graph Key: I239"@en-AU ;
    skos:definition "10 2  Dealing with things seized in exercising investigation powers"@en-AU ;
    skos:narrower F2021L00304:237 ;
    skos:prefLabel "Item I239"@en-AU ;
    dcat:accessURL <https://www.legislation.gov.au/F2021L00304/asmade/2021-03-24/text/original/epub/OEBPS/document_1/document_1.html#_Toc65844245> ;
    dcat:landingPage "https://www.legislation.gov.au/F2021L00304/asmade/2021-03-24/text/original/epub/OEBPS/document_1/document_1.html#_Toc65844245"^^xsd:anyURI ;
    dcat:theme legcons:Item .

F2021L00304:24 a legcons:Item,
        owl:Class,
        dcat:Resource ;
    rdfs:label "Item - I24 2 10  Instrument of exemption"@en-AU ;
    dct:isPartOf F2021L00304:10 ;
    dct:isReferencedBy F2021L00304: ;
    rdfs:comment "2 10  Instrument of exemption - Abrievated Graph Key: I24"@en-AU ;
    skos:definition "2 10  Instrument of exemption"@en-AU ;
    skos:narrower F2021L00304:10 ;
    skos:prefLabel "Item I24"@en-AU ;
    dcat:accessURL <https://www.legislation.gov.au/F2021L00304/asmade/2021-03-24/text/original/epub/OEBPS/document_1/document_1.html#_Toc65844030> ;
    dcat:landingPage "https://www.legislation.gov.au/F2021L00304/asmade/2021-03-24/text/original/epub/OEBPS/document_1/document_1.html#_Toc65844030"^^xsd:anyURI ;
    dcat:theme legcons:Item .

F2021L00304:242 a legcons:Item,
        owl:Class,
        dcat:Resource ;
    rdfs:label "Item - I242 11 1  Reviewable decisions"@en-AU ;
    dct:isPartOf F2021L00304:241 ;
    dct:isReferencedBy F2021L00304: ;
    rdfs:comment "11 1  Reviewable decisions - Abrievated Graph Key: I242"@en-AU ;
    skos:definition "11 1  Reviewable decisions"@en-AU ;
    skos:narrower F2021L00304:241 ;
    skos:prefLabel "Item I242"@en-AU ;
    dcat:accessURL <https://www.legislation.gov.au/F2021L00304/asmade/2021-03-24/text/original/epub/OEBPS/document_1/document_1.html#_Toc65844248> ;
    dcat:landingPage "https://www.legislation.gov.au/F2021L00304/asmade/2021-03-24/text/original/epub/OEBPS/document_1/document_1.html#_Toc65844248"^^xsd:anyURI ;
    dcat:theme legcons:Item .

F2021L00304:244 a legcons:Item,
        owl:Class,
        dcat:Resource ;
    rdfs:label "Item - I244 11 2  Purpose of this Part"@en-AU ;
    dct:isPartOf F2021L00304:243 ;
    dct:isReferencedBy F2021L00304: ;
    rdfs:comment "11 2  Purpose of this Part - Abrievated Graph Key: I244"@en-AU ;
    skos:definition "11 2  Purpose of this Part"@en-AU ;
    skos:narrower F2021L00304:243 ;
    skos:prefLabel "Item I244"@en-AU ;
    dcat:accessURL <https://www.legislation.gov.au/F2021L00304/asmade/2021-03-24/text/original/epub/OEBPS/document_1/document_1.html#_Toc65844250> ;
    dcat:landingPage "https://www.legislation.gov.au/F2021L00304/asmade/2021-03-24/text/original/epub/OEBPS/document_1/document_1.html#_Toc65844250"^^xsd:anyURI ;
    dcat:theme legcons:Item .

F2021L00304:245 a legcons:Item,
        owl:Class,
        dcat:Resource ;
    rdfs:label "Item - I245 11 3  General requirements for records"@en-AU ;
    dct:isPartOf F2021L00304:243 ;
    dct:isReferencedBy F2021L00304: ;
    rdfs:comment "11 3  General requirements for records - Abrievated Graph Key: I245"@en-AU ;
    skos:definition "11 3  General requirements for records"@en-AU ;
    skos:narrower F2021L00304:243 ;
    skos:prefLabel "Item I245"@en-AU ;
    dcat:accessURL <https://www.legislation.gov.au/F2021L00304/asmade/2021-03-24/text/original/epub/OEBPS/document_1/document_1.html#_Toc65844251> ;
    dcat:landingPage "https://www.legislation.gov.au/F2021L00304/asmade/2021-03-24/text/original/epub/OEBPS/document_1/document_1.html#_Toc65844251"^^xsd:anyURI ;
    dcat:theme legcons:Item .

F2021L00304:246 a legcons:Item,
        owl:Class,
        dcat:Resource ;
    rdfs:label "Item - I246 11 4  Government certificates"@en-AU ;
    dct:isPartOf F2021L00304:243 ;
    dct:isReferencedBy F2021L00304: ;
    rdfs:comment "11 4  Government certificates - Abrievated Graph Key: I246"@en-AU ;
    skos:definition "11 4  Government certificates"@en-AU ;
    skos:narrower F2021L00304:243 ;
    skos:prefLabel "Item I246"@en-AU ;
    dcat:accessURL <https://www.legislation.gov.au/F2021L00304/asmade/2021-03-24/text/original/epub/OEBPS/document_1/document_1.html#_Toc65844252> ;
    dcat:landingPage "https://www.legislation.gov.au/F2021L00304/asmade/2021-03-24/text/original/epub/OEBPS/document_1/document_1.html#_Toc65844252"^^xsd:anyURI ;
    dcat:theme legcons:Item .

F2021L00304:247 a legcons:Item,
        owl:Class,
        dcat:Resource ;
    rdfs:label "Item - I247 11 5  Export permits"@en-AU ;
    dct:isPartOf F2021L00304:243 ;
    dct:isReferencedBy F2021L00304: ;
    rdfs:comment "11 5  Export permits - Abrievated Graph Key: I247"@en-AU ;
    skos:definition "11 5  Export permits"@en-AU ;
    skos:narrower F2021L00304:243 ;
    skos:prefLabel "Item I247"@en-AU ;
    dcat:accessURL <https://www.legislation.gov.au/F2021L00304/asmade/2021-03-24/text/original/epub/OEBPS/document_1/document_1.html#_Toc65844253> ;
    dcat:landingPage "https://www.legislation.gov.au/F2021L00304/asmade/2021-03-24/text/original/epub/OEBPS/document_1/document_1.html#_Toc65844253"^^xsd:anyURI ;
    dcat:theme legcons:Item .

F2021L00304:248 a legcons:Item,
        owl:Class,
        dcat:Resource ;
    rdfs:label "Item - I248 11 6  Records to be retained by exporter"@en-AU ;
    dct:isPartOf F2021L00304:243 ;
    dct:isReferencedBy F2021L00304: ;
    rdfs:comment "11 6  Records to be retained by exporter - Abrievated Graph Key: I248"@en-AU ;
    skos:definition "11 6  Records to be retained by exporter"@en-AU ;
    skos:narrower F2021L00304:243 ;
    skos:prefLabel "Item I248"@en-AU ;
    dcat:accessURL <https://www.legislation.gov.au/F2021L00304/asmade/2021-03-24/text/original/epub/OEBPS/document_1/document_1.html#_Toc65844254> ;
    dcat:landingPage "https://www.legislation.gov.au/F2021L00304/asmade/2021-03-24/text/original/epub/OEBPS/document_1/document_1.html#_Toc65844254"^^xsd:anyURI ;
    dcat:theme legcons:Item .

F2021L00304:249 a legcons:Item,
        owl:Class,
        dcat:Resource ;
    rdfs:label "Item - I249 11 7  Records to be retained by occupier of registered establishment"@en-AU ;
    dct:isPartOf F2021L00304:243 ;
    dct:isReferencedBy F2021L00304: ;
    rdfs:comment "11 7  Records to be retained by occupier of registered establishment - Abrievated Graph Key: I249"@en-AU ;
    skos:definition "11 7  Records to be retained by occupier of registered establishment"@en-AU ;
    skos:narrower F2021L00304:243 ;
    skos:prefLabel "Item I249"@en-AU ;
    dcat:accessURL <https://www.legislation.gov.au/F2021L00304/asmade/2021-03-24/text/original/epub/OEBPS/document_1/document_1.html#_Toc65844255> ;
    dcat:landingPage "https://www.legislation.gov.au/F2021L00304/asmade/2021-03-24/text/original/epub/OEBPS/document_1/document_1.html#_Toc65844255"^^xsd:anyURI ;
    dcat:theme legcons:Item .

F2021L00304:25 a legcons:Item,
        owl:Class,
        dcat:Resource ;
    rdfs:label "Item - I25 2 11  Period of effect of exemption"@en-AU ;
    dct:isPartOf F2021L00304:10 ;
    dct:isReferencedBy F2021L00304: ;
    rdfs:comment "2 11  Period of effect of exemption - Abrievated Graph Key: I25"@en-AU ;
    skos:definition "2 11  Period of effect of exemption"@en-AU ;
    skos:narrower F2021L00304:10 ;
    skos:prefLabel "Item I25"@en-AU ;
    dcat:accessURL <https://www.legislation.gov.au/F2021L00304/asmade/2021-03-24/text/original/epub/OEBPS/document_1/document_1.html#_Toc65844031> ;
    dcat:landingPage "https://www.legislation.gov.au/F2021L00304/asmade/2021-03-24/text/original/epub/OEBPS/document_1/document_1.html#_Toc65844031"^^xsd:anyURI ;
    dcat:theme legcons:Item .

F2021L00304:250 a legcons:Item,
        owl:Class,
        dcat:Resource ;
    rdfs:label "Item - I250 11 8  Records to be retained by holder of approved arrangement"@en-AU ;
    dct:isPartOf F2021L00304:243 ;
    dct:isReferencedBy F2021L00304: ;
    rdfs:comment "11 8  Records to be retained by holder of approved arrangement - Abrievated Graph Key: I250"@en-AU ;
    skos:definition "11 8  Records to be retained by holder of approved arrangement"@en-AU ;
    skos:narrower F2021L00304:243 ;
    skos:prefLabel "Item I250"@en-AU ;
    dcat:accessURL <https://www.legislation.gov.au/F2021L00304/asmade/2021-03-24/text/original/epub/OEBPS/document_1/document_1.html#_Toc65844256> ;
    dcat:landingPage "https://www.legislation.gov.au/F2021L00304/asmade/2021-03-24/text/original/epub/OEBPS/document_1/document_1.html#_Toc65844256"^^xsd:anyURI ;
    dcat:theme legcons:Item .

F2021L00304:251 a legcons:Item,
        owl:Class,
        dcat:Resource ;
    rdfs:label "Item - I251 11 9  Records relating to official marking devices"@en-AU ;
    dct:isPartOf F2021L00304:243 ;
    dct:isReferencedBy F2021L00304: ;
    rdfs:comment "11 9  Records relating to official marking devices - Abrievated Graph Key: I251"@en-AU ;
    skos:definition "11 9  Records relating to official marking devices"@en-AU ;
    skos:narrower F2021L00304:243 ;
    skos:prefLabel "Item I251"@en-AU ;
    dcat:accessURL <https://www.legislation.gov.au/F2021L00304/asmade/2021-03-24/text/original/epub/OEBPS/document_1/document_1.html#_Toc65844257> ;
    dcat:landingPage "https://www.legislation.gov.au/F2021L00304/asmade/2021-03-24/text/original/epub/OEBPS/document_1/document_1.html#_Toc65844257"^^xsd:anyURI ;
    dcat:theme legcons:Item .

F2021L00304:252 a legcons:Item,
        owl:Class,
        dcat:Resource ;
    rdfs:label "Item - I252 11 10  Records must not be altered or defaced during retention period"@en-AU ;
    dct:isPartOf F2021L00304:243 ;
    dct:isReferencedBy F2021L00304: ;
    rdfs:comment "11 10  Records must not be altered or defaced during retention period - Abrievated Graph Key: I252"@en-AU ;
    skos:definition "11 10  Records must not be altered or defaced during retention period"@en-AU ;
    skos:narrower F2021L00304:243 ;
    skos:prefLabel "Item I252"@en-AU ;
    dcat:accessURL <https://www.legislation.gov.au/F2021L00304/asmade/2021-03-24/text/original/epub/OEBPS/document_1/document_1.html#_Toc65844258> ;
    dcat:landingPage "https://www.legislation.gov.au/F2021L00304/asmade/2021-03-24/text/original/epub/OEBPS/document_1/document_1.html#_Toc65844258"^^xsd:anyURI ;
    dcat:theme legcons:Item .

F2021L00304:254 a legcons:Item,
        owl:Class,
        dcat:Resource ;
    rdfs:label "Item - I254 11 11  Microbiological limitstaking testing and analysing samples"@en-AU ;
    dct:isPartOf F2021L00304:253 ;
    dct:isReferencedBy F2021L00304: ;
    rdfs:comment "11 11  Microbiological limitstaking testing and analysing samples - Abrievated Graph Key: I254"@en-AU ;
    skos:definition "11 11  Microbiological limitstaking testing and analysing samples"@en-AU ;
    skos:narrower F2021L00304:253 ;
    skos:prefLabel "Item I254"@en-AU ;
    dcat:accessURL <https://www.legislation.gov.au/F2021L00304/asmade/2021-03-24/text/original/epub/OEBPS/document_1/document_1.html#_Toc65844260> ;
    dcat:landingPage "https://www.legislation.gov.au/F2021L00304/asmade/2021-03-24/text/original/epub/OEBPS/document_1/document_1.html#_Toc65844260"^^xsd:anyURI ;
    dcat:theme legcons:Item .

F2021L00304:255 a legcons:Item,
        owl:Class,
        dcat:Resource ;
    rdfs:label "Item - I255 11 12  Storage of samples"@en-AU ;
    dct:isPartOf F2021L00304:253 ;
    dct:isReferencedBy F2021L00304: ;
    rdfs:comment "11 12  Storage of samples - Abrievated Graph Key: I255"@en-AU ;
    skos:definition "11 12  Storage of samples"@en-AU ;
    skos:narrower F2021L00304:253 ;
    skos:prefLabel "Item I255"@en-AU ;
    dcat:accessURL <https://www.legislation.gov.au/F2021L00304/asmade/2021-03-24/text/original/epub/OEBPS/document_1/document_1.html#_Toc65844261> ;
    dcat:landingPage "https://www.legislation.gov.au/F2021L00304/asmade/2021-03-24/text/original/epub/OEBPS/document_1/document_1.html#_Toc65844261"^^xsd:anyURI ;
    dcat:theme legcons:Item .

F2021L00304:257 a legcons:Item,
        owl:Class,
        dcat:Resource ;
    rdfs:label "Item - I257 11 13  Division of compensation between owners"@en-AU ;
    dct:isPartOf F2021L00304:256 ;
    dct:isReferencedBy F2021L00304: ;
    rdfs:comment "11 13  Division of compensation between owners - Abrievated Graph Key: I257"@en-AU ;
    skos:definition "11 13  Division of compensation between owners"@en-AU ;
    skos:narrower F2021L00304:256 ;
    skos:prefLabel "Item I257"@en-AU ;
    dcat:accessURL <https://www.legislation.gov.au/F2021L00304/asmade/2021-03-24/text/original/epub/OEBPS/document_1/document_1.html#_Toc65844263> ;
    dcat:landingPage "https://www.legislation.gov.au/F2021L00304/asmade/2021-03-24/text/original/epub/OEBPS/document_1/document_1.html#_Toc65844263"^^xsd:anyURI ;
    dcat:theme legcons:Item .

F2021L00304:258 a legcons:Item,
        owl:Class,
        dcat:Resource ;
    rdfs:label "Item - I258 11 14  Amount of compensation"@en-AU ;
    dct:isPartOf F2021L00304:256 ;
    dct:isReferencedBy F2021L00304: ;
    rdfs:comment "11 14  Amount of compensation - Abrievated Graph Key: I258"@en-AU ;
    skos:definition "11 14  Amount of compensation"@en-AU ;
    skos:narrower F2021L00304:256 ;
    skos:prefLabel "Item I258"@en-AU ;
    dcat:accessURL <https://www.legislation.gov.au/F2021L00304/asmade/2021-03-24/text/original/epub/OEBPS/document_1/document_1.html#_Toc65844264> ;
    dcat:landingPage "https://www.legislation.gov.au/F2021L00304/asmade/2021-03-24/text/original/epub/OEBPS/document_1/document_1.html#_Toc65844264"^^xsd:anyURI ;
    dcat:theme legcons:Item .

F2021L00304:26 a legcons:Item,
        owl:Class,
        dcat:Resource ;
    rdfs:label "Item - I26 2 12  Variation of conditions of exemptionmatters to which Secretary must have regard"@en-AU ;
    dct:isPartOf F2021L00304:10 ;
    dct:isReferencedBy F2021L00304: ;
    rdfs:comment "2 12  Variation of conditions of exemptionmatters to which Secretary must have regard - Abrievated Graph Key: I26"@en-AU ;
    skos:definition "2 12  Variation of conditions of exemptionmatters to which Secretary must have regard"@en-AU ;
    skos:narrower F2021L00304:10 ;
    skos:prefLabel "Item I26"@en-AU ;
    dcat:accessURL <https://www.legislation.gov.au/F2021L00304/asmade/2021-03-24/text/original/epub/OEBPS/document_1/document_1.html#_Toc65844032> ;
    dcat:landingPage "https://www.legislation.gov.au/F2021L00304/asmade/2021-03-24/text/original/epub/OEBPS/document_1/document_1.html#_Toc65844032"^^xsd:anyURI ;
    dcat:theme legcons:Item .

F2021L00304:260 a legcons:Item,
        owl:Class,
        dcat:Resource ;
    rdfs:label "Item - I260 11 15  Circumstances in which relevant Commonwealth liability of a person is taken to have been paid"@en-AU ;
    dct:isPartOf F2021L00304:259 ;
    dct:isReferencedBy F2021L00304: ;
    rdfs:comment "11 15  Circumstances in which relevant Commonwealth liability of a person is taken to have been paid - Abrievated Graph Key: I260"@en-AU ;
    skos:definition "11 15  Circumstances in which relevant Commonwealth liability of a person is taken to have been paid"@en-AU ;
    skos:narrower F2021L00304:259 ;
    skos:prefLabel "Item I260"@en-AU ;
    dcat:accessURL <https://www.legislation.gov.au/F2021L00304/asmade/2021-03-24/text/original/epub/OEBPS/document_1/document_1.html#_Toc65844266> ;
    dcat:landingPage "https://www.legislation.gov.au/F2021L00304/asmade/2021-03-24/text/original/epub/OEBPS/document_1/document_1.html#_Toc65844266"^^xsd:anyURI ;
    dcat:theme legcons:Item .

F2021L00304:263 a legcons:Item,
        owl:Class,
        dcat:Resource ;
    rdfs:label "Item - I263 12 1  Definitions"@en-AU ;
    dct:isPartOf F2021L00304:262 ;
    dct:isReferencedBy F2021L00304: ;
    rdfs:comment "12 1  Definitions - Abrievated Graph Key: I263"@en-AU ;
    skos:definition "12 1  Definitions"@en-AU ;
    skos:narrower F2021L00304:262 ;
    skos:prefLabel "Item I263"@en-AU ;
    dcat:accessURL <https://www.legislation.gov.au/F2021L00304/asmade/2021-03-24/text/original/epub/OEBPS/document_1/document_1.html#_Toc65844269> ;
    dcat:landingPage "https://www.legislation.gov.au/F2021L00304/asmade/2021-03-24/text/original/epub/OEBPS/document_1/document_1.html#_Toc65844269"^^xsd:anyURI ;
    dcat:theme legcons:Item .

F2021L00304:265 a legcons:Item,
        owl:Class,
        dcat:Resource ;
    rdfs:label "Item - I265 12 2  Information and declarations given before commencement time"@en-AU ;
    dct:isPartOf F2021L00304:264 ;
    dct:isReferencedBy F2021L00304: ;
    rdfs:comment "12 2  Information and declarations given before commencement time - Abrievated Graph Key: I265"@en-AU ;
    skos:definition "12 2  Information and declarations given before commencement time"@en-AU ;
    skos:narrower F2021L00304:264 ;
    skos:prefLabel "Item I265"@en-AU ;
    dcat:accessURL <https://www.legislation.gov.au/F2021L00304/asmade/2021-03-24/text/original/epub/OEBPS/document_1/document_1.html#_Toc65844271> ;
    dcat:landingPage "https://www.legislation.gov.au/F2021L00304/asmade/2021-03-24/text/original/epub/OEBPS/document_1/document_1.html#_Toc65844271"^^xsd:anyURI ;
    dcat:theme legcons:Item .

F2021L00304:268 a legcons:Item,
        owl:Class,
        dcat:Resource ;
    rdfs:label "Item - I268 12 3  Request for translation not complied with before commencement time"@en-AU ;
    dct:isPartOf F2021L00304:267 ;
    dct:isReferencedBy F2021L00304: ;
    rdfs:comment "12 3  Request for translation not complied with before commencement time - Abrievated Graph Key: I268"@en-AU ;
    skos:definition "12 3  Request for translation not complied with before commencement time"@en-AU ;
    skos:narrower F2021L00304:267 ;
    skos:prefLabel "Item I268"@en-AU ;
    dcat:accessURL <https://www.legislation.gov.au/F2021L00304/asmade/2021-03-24/text/original/epub/OEBPS/document_1/document_1.html#_Toc65844274> ;
    dcat:landingPage "https://www.legislation.gov.au/F2021L00304/asmade/2021-03-24/text/original/epub/OEBPS/document_1/document_1.html#_Toc65844274"^^xsd:anyURI ;
    dcat:theme legcons:Item .

F2021L00304:27 a legcons:Part,
        owl:Class,
        dcat:Resource ;
    rdfs:label "Part - P27 Part 3 Government certificates"@en-AU ;
    dct:isPartOf F2021L00304:10 ;
    dct:isReferencedBy F2021L00304: ;
    rdfs:comment "Part 3 Government certificates - Abrievated Graph Key: P27"@en-AU ;
    skos:definition "Part 3 Government certificates"@en-AU ;
    skos:narrower F2021L00304:10 ;
    skos:prefLabel "Part P27"@en-AU ;
    dcat:accessURL <https://www.legislation.gov.au/F2021L00304/asmade/2021-03-24/text/original/epub/OEBPS/document_1/document_1.html#_Toc65844033> ;
    dcat:landingPage "https://www.legislation.gov.au/F2021L00304/asmade/2021-03-24/text/original/epub/OEBPS/document_1/document_1.html#_Toc65844033"^^xsd:anyURI ;
    dcat:theme legcons:Part .

F2021L00304:270 a legcons:Item,
        owl:Class,
        dcat:Resource ;
    rdfs:label "Item - I270 12 4  Person approved before commencement time to manufacture an official mark"@en-AU ;
    dct:isPartOf F2021L00304:269 ;
    dct:isReferencedBy F2021L00304: ;
    rdfs:comment "12 4  Person approved before commencement time to manufacture an official mark - Abrievated Graph Key: I270"@en-AU ;
    skos:definition "12 4  Person approved before commencement time to manufacture an official mark"@en-AU ;
    skos:narrower F2021L00304:269 ;
    skos:prefLabel "Item I270"@en-AU ;
    dcat:accessURL <https://www.legislation.gov.au/F2021L00304/asmade/2021-03-24/text/original/epub/OEBPS/document_1/document_1.html#_Toc65844276> ;
    dcat:landingPage "https://www.legislation.gov.au/F2021L00304/asmade/2021-03-24/text/original/epub/OEBPS/document_1/document_1.html#_Toc65844276"^^xsd:anyURI ;
    dcat:theme legcons:Item .

F2021L00304:271 a legcons:Item,
        owl:Class,
        dcat:Resource ;
    rdfs:label "Item - I271 12 5  Person approved before commencement time to possess an official mark"@en-AU ;
    dct:isPartOf F2021L00304:269 ;
    dct:isReferencedBy F2021L00304: ;
    rdfs:comment "12 5  Person approved before commencement time to possess an official mark - Abrievated Graph Key: I271"@en-AU ;
    skos:definition "12 5  Person approved before commencement time to possess an official mark"@en-AU ;
    skos:narrower F2021L00304:269 ;
    skos:prefLabel "Item I271"@en-AU ;
    dcat:accessURL <https://www.legislation.gov.au/F2021L00304/asmade/2021-03-24/text/original/epub/OEBPS/document_1/document_1.html#_Toc65844277> ;
    dcat:landingPage "https://www.legislation.gov.au/F2021L00304/asmade/2021-03-24/text/original/epub/OEBPS/document_1/document_1.html#_Toc65844277"^^xsd:anyURI ;
    dcat:theme legcons:Item .

F2021L00304:272 a legcons:Item,
        owl:Class,
        dcat:Resource ;
    rdfs:label "Item - I272 12 6  Person approved before commencement time to apply an official mark"@en-AU ;
    dct:isPartOf F2021L00304:269 ;
    dct:isReferencedBy F2021L00304: ;
    rdfs:comment "12 6  Person approved before commencement time to apply an official mark - Abrievated Graph Key: I272"@en-AU ;
    skos:definition "12 6  Person approved before commencement time to apply an official mark"@en-AU ;
    skos:narrower F2021L00304:269 ;
    skos:prefLabel "Item I272"@en-AU ;
    dcat:accessURL <https://www.legislation.gov.au/F2021L00304/asmade/2021-03-24/text/original/epub/OEBPS/document_1/document_1.html#_Toc65844278> ;
    dcat:landingPage "https://www.legislation.gov.au/F2021L00304/asmade/2021-03-24/text/original/epub/OEBPS/document_1/document_1.html#_Toc65844278"^^xsd:anyURI ;
    dcat:theme legcons:Item .

F2021L00304:274 a legcons:Item,
        owl:Class,
        dcat:Resource ;
    rdfs:label "Item - I274 12 7  Person approved before commencement time to manufacture an official marking device"@en-AU ;
    dct:isPartOf F2021L00304:273 ;
    dct:isReferencedBy F2021L00304: ;
    rdfs:comment "12 7  Person approved before commencement time to manufacture an official marking device - Abrievated Graph Key: I274"@en-AU ;
    skos:definition "12 7  Person approved before commencement time to manufacture an official marking device"@en-AU ;
    skos:narrower F2021L00304:273 ;
    skos:prefLabel "Item I274"@en-AU ;
    dcat:accessURL <https://www.legislation.gov.au/F2021L00304/asmade/2021-03-24/text/original/epub/OEBPS/document_1/document_1.html#_Toc65844280> ;
    dcat:landingPage "https://www.legislation.gov.au/F2021L00304/asmade/2021-03-24/text/original/epub/OEBPS/document_1/document_1.html#_Toc65844280"^^xsd:anyURI ;
    dcat:theme legcons:Item .

F2021L00304:275 a legcons:Item,
        owl:Class,
        dcat:Resource ;
    rdfs:label "Item - I275 12 8  Person approved before commencement time to possess an official marking device"@en-AU ;
    dct:isPartOf F2021L00304:273 ;
    dct:isReferencedBy F2021L00304: ;
    rdfs:comment "12 8  Person approved before commencement time to possess an official marking device - Abrievated Graph Key: I275"@en-AU ;
    skos:definition "12 8  Person approved before commencement time to possess an official marking device"@en-AU ;
    skos:narrower F2021L00304:273 ;
    skos:prefLabel "Item I275"@en-AU ;
    dcat:accessURL <https://www.legislation.gov.au/F2021L00304/asmade/2021-03-24/text/original/epub/OEBPS/document_1/document_1.html#_Toc65844281> ;
    dcat:landingPage "https://www.legislation.gov.au/F2021L00304/asmade/2021-03-24/text/original/epub/OEBPS/document_1/document_1.html#_Toc65844281"^^xsd:anyURI ;
    dcat:theme legcons:Item .

F2021L00304:278 a legcons:Item,
        owl:Class,
        dcat:Resource ;
    rdfs:label "Item - I278 12 9  Application for approval as auditor not decided or notice of decision not given before commencement time"@en-AU ;
    dct:isPartOf F2021L00304:277 ;
    dct:isReferencedBy F2021L00304: ;
    rdfs:comment "12 9  Application for approval as auditor not decided or notice of decision not given before commencement time - Abrievated Graph Key: I278"@en-AU ;
    skos:definition "12 9  Application for approval as auditor not decided or notice of decision not given before commencement time"@en-AU ;
    skos:narrower F2021L00304:277 ;
    skos:prefLabel "Item I278"@en-AU ;
    dcat:accessURL <https://www.legislation.gov.au/F2021L00304/asmade/2021-03-24/text/original/epub/OEBPS/document_1/document_1.html#_Toc65844284> ;
    dcat:landingPage "https://www.legislation.gov.au/F2021L00304/asmade/2021-03-24/text/original/epub/OEBPS/document_1/document_1.html#_Toc65844284"^^xsd:anyURI ;
    dcat:theme legcons:Item .

F2021L00304:279 a legcons:Item,
        owl:Class,
        dcat:Resource ;
    rdfs:label "Item - I279 12 10  Request for further information not complied with before commencement time"@en-AU ;
    dct:isPartOf F2021L00304:277 ;
    dct:isReferencedBy F2021L00304: ;
    rdfs:comment "12 10  Request for further information not complied with before commencement time - Abrievated Graph Key: I279"@en-AU ;
    skos:definition "12 10  Request for further information not complied with before commencement time"@en-AU ;
    skos:narrower F2021L00304:277 ;
    skos:prefLabel "Item I279"@en-AU ;
    dcat:accessURL <https://www.legislation.gov.au/F2021L00304/asmade/2021-03-24/text/original/epub/OEBPS/document_1/document_1.html#_Toc65844285> ;
    dcat:landingPage "https://www.legislation.gov.au/F2021L00304/asmade/2021-03-24/text/original/epub/OEBPS/document_1/document_1.html#_Toc65844285"^^xsd:anyURI ;
    dcat:theme legcons:Item .

F2021L00304:28 a legcons:Item,
        owl:Class,
        dcat:Resource ;
    rdfs:label "Item - I28 2 13  When government certificate may be issued in relation to milk or milk products"@en-AU ;
    dct:isPartOf F2021L00304:10 ;
    dct:isReferencedBy F2021L00304: ;
    rdfs:comment "2 13  When government certificate may be issued in relation to milk or milk products - Abrievated Graph Key: I28"@en-AU ;
    skos:definition "2 13  When government certificate may be issued in relation to milk or milk products"@en-AU ;
    skos:narrower F2021L00304:10 ;
    skos:prefLabel "Item I28"@en-AU ;
    dcat:accessURL <https://www.legislation.gov.au/F2021L00304/asmade/2021-03-24/text/original/epub/OEBPS/document_1/document_1.html#_Toc65844034> ;
    dcat:landingPage "https://www.legislation.gov.au/F2021L00304/asmade/2021-03-24/text/original/epub/OEBPS/document_1/document_1.html#_Toc65844034"^^xsd:anyURI ;
    dcat:theme legcons:Item .

F2021L00304:280 a legcons:Item,
        owl:Class,
        dcat:Resource ;
    rdfs:label "Item - I280 12 11  Decision to revoke approval as auditor decided but notice not given before commencement time"@en-AU ;
    dct:isPartOf F2021L00304:277 ;
    dct:isReferencedBy F2021L00304: ;
    rdfs:comment "12 11  Decision to revoke approval as auditor decided but notice not given before commencement time - Abrievated Graph Key: I280"@en-AU ;
    skos:definition "12 11  Decision to revoke approval as auditor decided but notice not given before commencement time"@en-AU ;
    skos:narrower F2021L00304:277 ;
    skos:prefLabel "Item I280"@en-AU ;
    dcat:accessURL <https://www.legislation.gov.au/F2021L00304/asmade/2021-03-24/text/original/epub/OEBPS/document_1/document_1.html#_Toc65844286> ;
    dcat:landingPage "https://www.legislation.gov.au/F2021L00304/asmade/2021-03-24/text/original/epub/OEBPS/document_1/document_1.html#_Toc65844286"^^xsd:anyURI ;
    dcat:theme legcons:Item .

F2021L00304:282 a legcons:Item,
        owl:Class,
        dcat:Resource ;
    rdfs:label "Item - I282 12 12  Verification by authorised officer before commencement time"@en-AU ;
    dct:isPartOf F2021L00304:281 ;
    dct:isReferencedBy F2021L00304: ;
    rdfs:comment "12 12  Verification by authorised officer before commencement time - Abrievated Graph Key: I282"@en-AU ;
    skos:definition "12 12  Verification by authorised officer before commencement time"@en-AU ;
    skos:narrower F2021L00304:281 ;
    skos:prefLabel "Item I282"@en-AU ;
    dcat:accessURL <https://www.legislation.gov.au/F2021L00304/asmade/2021-03-24/text/original/epub/OEBPS/document_1/document_1.html#_Toc65844288> ;
    dcat:landingPage "https://www.legislation.gov.au/F2021L00304/asmade/2021-03-24/text/original/epub/OEBPS/document_1/document_1.html#_Toc65844288"^^xsd:anyURI ;
    dcat:theme legcons:Item .

F2021L00304:29 a legcons:Item,
        owl:Class,
        dcat:Resource ;
    rdfs:label "Item - I29 2 14  Matters stated in government certificatemanufacturing grade milk or milk products"@en-AU ;
    dct:isPartOf F2021L00304:10 ;
    dct:isReferencedBy F2021L00304: ;
    rdfs:comment "2 14  Matters stated in government certificatemanufacturing grade milk or milk products - Abrievated Graph Key: I29"@en-AU ;
    skos:definition "2 14  Matters stated in government certificatemanufacturing grade milk or milk products"@en-AU ;
    skos:narrower F2021L00304:10 ;
    skos:prefLabel "Item I29"@en-AU ;
    dcat:accessURL <https://www.legislation.gov.au/F2021L00304/asmade/2021-03-24/text/original/epub/OEBPS/document_1/document_1.html#_Toc65844035> ;
    dcat:landingPage "https://www.legislation.gov.au/F2021L00304/asmade/2021-03-24/text/original/epub/OEBPS/document_1/document_1.html#_Toc65844035"^^xsd:anyURI ;
    dcat:theme legcons:Item .

F2021L00304:3 a legcons:Item,
        owl:Class,
        dcat:Resource ;
    rdfs:label "Item - I3 1 1  Name"@en-AU ;
    dct:isPartOf F2021L00304:1 ;
    dct:isReferencedBy F2021L00304: ;
    rdfs:comment "1 1  Name - Abrievated Graph Key: I3"@en-AU ;
    skos:definition "1 1  Name"@en-AU ;
    skos:narrower F2021L00304:1 ;
    skos:prefLabel "Item I3"@en-AU ;
    dcat:accessURL <https://www.legislation.gov.au/F2021L00304/asmade/2021-03-24/text/original/epub/OEBPS/document_1/document_1.html#_Toc65844009> ;
    dcat:landingPage "https://www.legislation.gov.au/F2021L00304/asmade/2021-03-24/text/original/epub/OEBPS/document_1/document_1.html#_Toc65844009"^^xsd:anyURI ;
    dcat:theme legcons:Item .

F2021L00304:30 a legcons:Item,
        owl:Class,
        dcat:Resource ;
    rdfs:label "Item - I30 2 15  Requirements before issue of government certificatecondition of milk or milk products"@en-AU ;
    dct:isPartOf F2021L00304:10 ;
    dct:isReferencedBy F2021L00304: ;
    rdfs:comment "2 15  Requirements before issue of government certificatecondition of milk or milk products - Abrievated Graph Key: I30"@en-AU ;
    skos:definition "2 15  Requirements before issue of government certificatecondition of milk or milk products"@en-AU ;
    skos:narrower F2021L00304:10 ;
    skos:prefLabel "Item I30"@en-AU ;
    dcat:accessURL <https://www.legislation.gov.au/F2021L00304/asmade/2021-03-24/text/original/epub/OEBPS/document_1/document_1.html#_Toc65844036> ;
    dcat:landingPage "https://www.legislation.gov.au/F2021L00304/asmade/2021-03-24/text/original/epub/OEBPS/document_1/document_1.html#_Toc65844036"^^xsd:anyURI ;
    dcat:theme legcons:Item .

F2021L00304:31 a legcons:Item,
        owl:Class,
        dcat:Resource ;
    rdfs:label "Item - I31 2 16  Circumstances for refusing to issue government certificate"@en-AU ;
    dct:isPartOf F2021L00304:10 ;
    dct:isReferencedBy F2021L00304: ;
    rdfs:comment "2 16  Circumstances for refusing to issue government certificate - Abrievated Graph Key: I31"@en-AU ;
    skos:definition "2 16  Circumstances for refusing to issue government certificate"@en-AU ;
    skos:narrower F2021L00304:10 ;
    skos:prefLabel "Item I31"@en-AU ;
    dcat:accessURL <https://www.legislation.gov.au/F2021L00304/asmade/2021-03-24/text/original/epub/OEBPS/document_1/document_1.html#_Toc65844037> ;
    dcat:landingPage "https://www.legislation.gov.au/F2021L00304/asmade/2021-03-24/text/original/epub/OEBPS/document_1/document_1.html#_Toc65844037"^^xsd:anyURI ;
    dcat:theme legcons:Item .

F2021L00304:32 a legcons:Item,
        owl:Class,
        dcat:Resource ;
    rdfs:label "Item - I32 2 17  Changes that require holder of certificate to give additional or corrected information to the issuing body"@en-AU ;
    dct:isPartOf F2021L00304:10 ;
    dct:isReferencedBy F2021L00304: ;
    rdfs:comment "2 17  Changes that require holder of certificate to give additional or corrected information to the issuing body - Abrievated Graph Key: I32"@en-AU ;
    skos:definition "2 17  Changes that require holder of certificate to give additional or corrected information to the issuing body"@en-AU ;
    skos:narrower F2021L00304:10 ;
    skos:prefLabel "Item I32"@en-AU ;
    dcat:accessURL <https://www.legislation.gov.au/F2021L00304/asmade/2021-03-24/text/original/epub/OEBPS/document_1/document_1.html#_Toc65844038> ;
    dcat:landingPage "https://www.legislation.gov.au/F2021L00304/asmade/2021-03-24/text/original/epub/OEBPS/document_1/document_1.html#_Toc65844038"^^xsd:anyURI ;
    dcat:theme legcons:Item .

F2021L00304:33 a legcons:Item,
        owl:Class,
        dcat:Resource ;
    rdfs:label "Item - I33 2 18  Return of government certificate"@en-AU ;
    dct:isPartOf F2021L00304:10 ;
    dct:isReferencedBy F2021L00304: ;
    rdfs:comment "2 18  Return of government certificate - Abrievated Graph Key: I33"@en-AU ;
    skos:definition "2 18  Return of government certificate"@en-AU ;
    skos:narrower F2021L00304:10 ;
    skos:prefLabel "Item I33"@en-AU ;
    dcat:accessURL <https://www.legislation.gov.au/F2021L00304/asmade/2021-03-24/text/original/epub/OEBPS/document_1/document_1.html#_Toc65844039> ;
    dcat:landingPage "https://www.legislation.gov.au/F2021L00304/asmade/2021-03-24/text/original/epub/OEBPS/document_1/document_1.html#_Toc65844039"^^xsd:anyURI ;
    dcat:theme legcons:Item .

F2021L00304:37 a legcons:Item,
        owl:Class,
        dcat:Resource ;
    rdfs:label "Item - I37 4 1  Purpose of this Division"@en-AU ;
    dct:isPartOf F2021L00304:36 ;
    dct:isReferencedBy F2021L00304: ;
    rdfs:comment "4 1  Purpose of this Division - Abrievated Graph Key: I37"@en-AU ;
    skos:definition "4 1  Purpose of this Division"@en-AU ;
    skos:narrower F2021L00304:36 ;
    skos:prefLabel "Item I37"@en-AU ;
    dcat:accessURL <https://www.legislation.gov.au/F2021L00304/asmade/2021-03-24/text/original/epub/OEBPS/document_1/document_1.html#_Toc65844043> ;
    dcat:landingPage "https://www.legislation.gov.au/F2021L00304/asmade/2021-03-24/text/original/epub/OEBPS/document_1/document_1.html#_Toc65844043"^^xsd:anyURI ;
    dcat:theme legcons:Item .

F2021L00304:38 a legcons:Item,
        owl:Class,
        dcat:Resource ;
    rdfs:label "Item - I38 4 2  Equipment facilities and essential servicesgeneral"@en-AU ;
    dct:isPartOf F2021L00304:36 ;
    dct:isReferencedBy F2021L00304: ;
    rdfs:comment "4 2  Equipment facilities and essential servicesgeneral - Abrievated Graph Key: I38"@en-AU ;
    skos:definition "4 2  Equipment facilities and essential servicesgeneral"@en-AU ;
    skos:narrower F2021L00304:36 ;
    skos:prefLabel "Item I38"@en-AU ;
    dcat:accessURL <https://www.legislation.gov.au/F2021L00304/asmade/2021-03-24/text/original/epub/OEBPS/document_1/document_1.html#_Toc65844044> ;
    dcat:landingPage "https://www.legislation.gov.au/F2021L00304/asmade/2021-03-24/text/original/epub/OEBPS/document_1/document_1.html#_Toc65844044"^^xsd:anyURI ;
    dcat:theme legcons:Item .

F2021L00304:39 a legcons:Item,
        owl:Class,
        dcat:Resource ;
    rdfs:label "Item - I39 4 3  Measuring devices"@en-AU ;
    dct:isPartOf F2021L00304:36 ;
    dct:isReferencedBy F2021L00304: ;
    rdfs:comment "4 3  Measuring devices - Abrievated Graph Key: I39"@en-AU ;
    skos:definition "4 3  Measuring devices"@en-AU ;
    skos:narrower F2021L00304:36 ;
    skos:prefLabel "Item I39"@en-AU ;
    dcat:accessURL <https://www.legislation.gov.au/F2021L00304/asmade/2021-03-24/text/original/epub/OEBPS/document_1/document_1.html#_Toc65844045> ;
    dcat:landingPage "https://www.legislation.gov.au/F2021L00304/asmade/2021-03-24/text/original/epub/OEBPS/document_1/document_1.html#_Toc65844045"^^xsd:anyURI ;
    dcat:theme legcons:Item .

F2021L00304:4 a legcons:Item,
        owl:Class,
        dcat:Resource ;
    rdfs:label "Item - I4 1 2  Commencement"@en-AU ;
    dct:isPartOf F2021L00304:1 ;
    dct:isReferencedBy F2021L00304: ;
    rdfs:comment "1 2  Commencement - Abrievated Graph Key: I4"@en-AU ;
    skos:definition "1 2  Commencement"@en-AU ;
    skos:narrower F2021L00304:1 ;
    skos:prefLabel "Item I4"@en-AU ;
    dcat:accessURL <https://www.legislation.gov.au/F2021L00304/asmade/2021-03-24/text/original/epub/OEBPS/document_1/document_1.html#_Toc65844010> ;
    dcat:landingPage "https://www.legislation.gov.au/F2021L00304/asmade/2021-03-24/text/original/epub/OEBPS/document_1/document_1.html#_Toc65844010"^^xsd:anyURI ;
    dcat:theme legcons:Item .

F2021L00304:40 a legcons:Item,
        owl:Class,
        dcat:Resource ;
    rdfs:label "Item - I40 4 4  Establishment including construction"@en-AU ;
    dct:isPartOf F2021L00304:36 ;
    dct:isReferencedBy F2021L00304: ;
    rdfs:comment "4 4  Establishment including construction - Abrievated Graph Key: I40"@en-AU ;
    skos:definition "4 4  Establishment including construction"@en-AU ;
    skos:narrower F2021L00304:36 ;
    skos:prefLabel "Item I40"@en-AU ;
    dcat:accessURL <https://www.legislation.gov.au/F2021L00304/asmade/2021-03-24/text/original/epub/OEBPS/document_1/document_1.html#_Toc65844046> ;
    dcat:landingPage "https://www.legislation.gov.au/F2021L00304/asmade/2021-03-24/text/original/epub/OEBPS/document_1/document_1.html#_Toc65844046"^^xsd:anyURI ;
    dcat:theme legcons:Item .

F2021L00304:41 a legcons:Item,
        owl:Class,
        dcat:Resource ;
    rdfs:label "Item - I41 4 5  Fixtures fittings and equipment"@en-AU ;
    dct:isPartOf F2021L00304:36 ;
    dct:isReferencedBy F2021L00304: ;
    rdfs:comment "4 5  Fixtures fittings and equipment - Abrievated Graph Key: I41"@en-AU ;
    skos:definition "4 5  Fixtures fittings and equipment"@en-AU ;
    skos:narrower F2021L00304:36 ;
    skos:prefLabel "Item I41"@en-AU ;
    dcat:accessURL <https://www.legislation.gov.au/F2021L00304/asmade/2021-03-24/text/original/epub/OEBPS/document_1/document_1.html#_Toc65844047> ;
    dcat:landingPage "https://www.legislation.gov.au/F2021L00304/asmade/2021-03-24/text/original/epub/OEBPS/document_1/document_1.html#_Toc65844047"^^xsd:anyURI ;
    dcat:theme legcons:Item .

F2021L00304:42 a legcons:Item,
        owl:Class,
        dcat:Resource ;
    rdfs:label "Item - I42 4 6  Storage facilities for items other than milk or milk products"@en-AU ;
    dct:isPartOf F2021L00304:36 ;
    dct:isReferencedBy F2021L00304: ;
    rdfs:comment "4 6  Storage facilities for items other than milk or milk products - Abrievated Graph Key: I42"@en-AU ;
    skos:definition "4 6  Storage facilities for items other than milk or milk products"@en-AU ;
    skos:narrower F2021L00304:36 ;
    skos:prefLabel "Item I42"@en-AU ;
    dcat:accessURL <https://www.legislation.gov.au/F2021L00304/asmade/2021-03-24/text/original/epub/OEBPS/document_1/document_1.html#_Toc65844048> ;
    dcat:landingPage "https://www.legislation.gov.au/F2021L00304/asmade/2021-03-24/text/original/epub/OEBPS/document_1/document_1.html#_Toc65844048"^^xsd:anyURI ;
    dcat:theme legcons:Item .

F2021L00304:43 a legcons:Item,
        owl:Class,
        dcat:Resource ;
    rdfs:label "Item - I43 4 7  Cleaning and sanitising facilities"@en-AU ;
    dct:isPartOf F2021L00304:36 ;
    dct:isReferencedBy F2021L00304: ;
    rdfs:comment "4 7  Cleaning and sanitising facilities - Abrievated Graph Key: I43"@en-AU ;
    skos:definition "4 7  Cleaning and sanitising facilities"@en-AU ;
    skos:narrower F2021L00304:36 ;
    skos:prefLabel "Item I43"@en-AU ;
    dcat:accessURL <https://www.legislation.gov.au/F2021L00304/asmade/2021-03-24/text/original/epub/OEBPS/document_1/document_1.html#_Toc65844049> ;
    dcat:landingPage "https://www.legislation.gov.au/F2021L00304/asmade/2021-03-24/text/original/epub/OEBPS/document_1/document_1.html#_Toc65844049"^^xsd:anyURI ;
    dcat:theme legcons:Item .

F2021L00304:44 a legcons:Item,
        owl:Class,
        dcat:Resource ;
    rdfs:label "Item - I44 4 8  Amenities"@en-AU ;
    dct:isPartOf F2021L00304:36 ;
    dct:isReferencedBy F2021L00304: ;
    rdfs:comment "4 8  Amenities - Abrievated Graph Key: I44"@en-AU ;
    skos:definition "4 8  Amenities"@en-AU ;
    skos:narrower F2021L00304:36 ;
    skos:prefLabel "Item I44"@en-AU ;
    dcat:accessURL <https://www.legislation.gov.au/F2021L00304/asmade/2021-03-24/text/original/epub/OEBPS/document_1/document_1.html#_Toc65844050> ;
    dcat:landingPage "https://www.legislation.gov.au/F2021L00304/asmade/2021-03-24/text/original/epub/OEBPS/document_1/document_1.html#_Toc65844050"^^xsd:anyURI ;
    dcat:theme legcons:Item .

F2021L00304:45 a legcons:Item,
        owl:Class,
        dcat:Resource ;
    rdfs:label "Item - I45 4 9  Essential services"@en-AU ;
    dct:isPartOf F2021L00304:36 ;
    dct:isReferencedBy F2021L00304: ;
    rdfs:comment "4 9  Essential services - Abrievated Graph Key: I45"@en-AU ;
    skos:definition "4 9  Essential services"@en-AU ;
    skos:narrower F2021L00304:36 ;
    skos:prefLabel "Item I45"@en-AU ;
    dcat:accessURL <https://www.legislation.gov.au/F2021L00304/asmade/2021-03-24/text/original/epub/OEBPS/document_1/document_1.html#_Toc65844051> ;
    dcat:landingPage "https://www.legislation.gov.au/F2021L00304/asmade/2021-03-24/text/original/epub/OEBPS/document_1/document_1.html#_Toc65844051"^^xsd:anyURI ;
    dcat:theme legcons:Item .

F2021L00304:47 a legcons:Item,
        owl:Class,
        dcat:Resource ;
    rdfs:label "Item - I47 4 10  Purpose of this Division"@en-AU ;
    dct:isPartOf F2021L00304:46 ;
    dct:isReferencedBy F2021L00304: ;
    rdfs:comment "4 10  Purpose of this Division - Abrievated Graph Key: I47"@en-AU ;
    skos:definition "4 10  Purpose of this Division"@en-AU ;
    skos:narrower F2021L00304:46 ;
    skos:prefLabel "Item I47"@en-AU ;
    dcat:accessURL <https://www.legislation.gov.au/F2021L00304/asmade/2021-03-24/text/original/epub/OEBPS/document_1/document_1.html#_Toc65844053> ;
    dcat:landingPage "https://www.legislation.gov.au/F2021L00304/asmade/2021-03-24/text/original/epub/OEBPS/document_1/document_1.html#_Toc65844053"^^xsd:anyURI ;
    dcat:theme legcons:Item .

F2021L00304:48 a legcons:Item,
        owl:Class,
        dcat:Resource ;
    rdfs:label "Item - I48 4 11  Operations must be carried out in a way that will ensure requirements of the Act are met"@en-AU ;
    dct:isPartOf F2021L00304:46 ;
    dct:isReferencedBy F2021L00304: ;
    rdfs:comment "4 11  Operations must be carried out in a way that will ensure requirements of the Act are met - Abrievated Graph Key: I48"@en-AU ;
    skos:definition "4 11  Operations must be carried out in a way that will ensure requirements of the Act are met"@en-AU ;
    skos:narrower F2021L00304:46 ;
    skos:prefLabel "Item I48"@en-AU ;
    dcat:accessURL <https://www.legislation.gov.au/F2021L00304/asmade/2021-03-24/text/original/epub/OEBPS/document_1/document_1.html#_Toc65844054> ;
    dcat:landingPage "https://www.legislation.gov.au/F2021L00304/asmade/2021-03-24/text/original/epub/OEBPS/document_1/document_1.html#_Toc65844054"^^xsd:anyURI ;
    dcat:theme legcons:Item .

F2021L00304:5 a legcons:Item,
        owl:Class,
        dcat:Resource ;
    rdfs:label "Item - I5 1 3  Authority"@en-AU ;
    dct:isPartOf F2021L00304:1 ;
    dct:isReferencedBy F2021L00304: ;
    rdfs:comment "1 3  Authority - Abrievated Graph Key: I5"@en-AU ;
    skos:definition "1 3  Authority"@en-AU ;
    skos:narrower F2021L00304:1 ;
    skos:prefLabel "Item I5"@en-AU ;
    dcat:accessURL <https://www.legislation.gov.au/F2021L00304/asmade/2021-03-24/text/original/epub/OEBPS/document_1/document_1.html#_Toc65844011> ;
    dcat:landingPage "https://www.legislation.gov.au/F2021L00304/asmade/2021-03-24/text/original/epub/OEBPS/document_1/document_1.html#_Toc65844011"^^xsd:anyURI ;
    dcat:theme legcons:Item .

F2021L00304:50 a legcons:Item,
        owl:Class,
        dcat:Resource ;
    rdfs:label "Item - I50 4 12  Purpose of this Part"@en-AU ;
    dct:isPartOf F2021L00304:49 ;
    dct:isReferencedBy F2021L00304: ;
    rdfs:comment "4 12  Purpose of this Part - Abrievated Graph Key: I50"@en-AU ;
    skos:definition "4 12  Purpose of this Part"@en-AU ;
    skos:narrower F2021L00304:49 ;
    skos:prefLabel "Item I50"@en-AU ;
    dcat:accessURL <https://www.legislation.gov.au/F2021L00304/asmade/2021-03-24/text/original/epub/OEBPS/document_1/document_1.html#_Toc65844056> ;
    dcat:landingPage "https://www.legislation.gov.au/F2021L00304/asmade/2021-03-24/text/original/epub/OEBPS/document_1/document_1.html#_Toc65844056"^^xsd:anyURI ;
    dcat:theme legcons:Item .

F2021L00304:51 a legcons:Item,
        owl:Class,
        dcat:Resource ;
    rdfs:label "Item - I51 4 13  Requirements for registration continue to be met"@en-AU ;
    dct:isPartOf F2021L00304:49 ;
    dct:isReferencedBy F2021L00304: ;
    rdfs:comment "4 13  Requirements for registration continue to be met - Abrievated Graph Key: I51"@en-AU ;
    skos:definition "4 13  Requirements for registration continue to be met"@en-AU ;
    skos:narrower F2021L00304:49 ;
    skos:prefLabel "Item I51"@en-AU ;
    dcat:accessURL <https://www.legislation.gov.au/F2021L00304/asmade/2021-03-24/text/original/epub/OEBPS/document_1/document_1.html#_Toc65844057> ;
    dcat:landingPage "https://www.legislation.gov.au/F2021L00304/asmade/2021-03-24/text/original/epub/OEBPS/document_1/document_1.html#_Toc65844057"^^xsd:anyURI ;
    dcat:theme legcons:Item .

F2021L00304:52 a legcons:Item,
        owl:Class,
        dcat:Resource ;
    rdfs:label "Item - I52 4 14  Other operational hygiene requirements"@en-AU ;
    dct:isPartOf F2021L00304:49 ;
    dct:isReferencedBy F2021L00304: ;
    rdfs:comment "4 14  Other operational hygiene requirements - Abrievated Graph Key: I52"@en-AU ;
    skos:definition "4 14  Other operational hygiene requirements"@en-AU ;
    skos:narrower F2021L00304:49 ;
    skos:prefLabel "Item I52"@en-AU ;
    dcat:accessURL <https://www.legislation.gov.au/F2021L00304/asmade/2021-03-24/text/original/epub/OEBPS/document_1/document_1.html#_Toc65844058> ;
    dcat:landingPage "https://www.legislation.gov.au/F2021L00304/asmade/2021-03-24/text/original/epub/OEBPS/document_1/document_1.html#_Toc65844058"^^xsd:anyURI ;
    dcat:theme legcons:Item .

F2021L00304:54 a legcons:Item,
        owl:Class,
        dcat:Resource ;
    rdfs:label "Item - I54 4 15  Period within which application to renew registration must be made"@en-AU ;
    dct:isPartOf F2021L00304:53 ;
    dct:isReferencedBy F2021L00304: ;
    rdfs:comment "4 15  Period within which application to renew registration must be made - Abrievated Graph Key: I54"@en-AU ;
    skos:definition "4 15  Period within which application to renew registration must be made"@en-AU ;
    skos:narrower F2021L00304:53 ;
    skos:prefLabel "Item I54"@en-AU ;
    dcat:accessURL <https://www.legislation.gov.au/F2021L00304/asmade/2021-03-24/text/original/epub/OEBPS/document_1/document_1.html#_Toc65844060> ;
    dcat:landingPage "https://www.legislation.gov.au/F2021L00304/asmade/2021-03-24/text/original/epub/OEBPS/document_1/document_1.html#_Toc65844060"^^xsd:anyURI ;
    dcat:theme legcons:Item .

F2021L00304:55 a legcons:Item,
        owl:Class,
        dcat:Resource ;
    rdfs:label "Item - I55 4 16  Requirements for renewal of registration"@en-AU ;
    dct:isPartOf F2021L00304:53 ;
    dct:isReferencedBy F2021L00304: ;
    rdfs:comment "4 16  Requirements for renewal of registration - Abrievated Graph Key: I55"@en-AU ;
    skos:definition "4 16  Requirements for renewal of registration"@en-AU ;
    skos:narrower F2021L00304:53 ;
    skos:prefLabel "Item I55"@en-AU ;
    dcat:accessURL <https://www.legislation.gov.au/F2021L00304/asmade/2021-03-24/text/original/epub/OEBPS/document_1/document_1.html#_Toc65844061> ;
    dcat:landingPage "https://www.legislation.gov.au/F2021L00304/asmade/2021-03-24/text/original/epub/OEBPS/document_1/document_1.html#_Toc65844061"^^xsd:anyURI ;
    dcat:theme legcons:Item .

F2021L00304:57 a legcons:Item,
        owl:Class,
        dcat:Resource ;
    rdfs:label "Item - I57 4 17  Request by occupier for suspension"@en-AU ;
    dct:isPartOf F2021L00304:56 ;
    dct:isReferencedBy F2021L00304: ;
    rdfs:comment "4 17  Request by occupier for suspension - Abrievated Graph Key: I57"@en-AU ;
    skos:definition "4 17  Request by occupier for suspension"@en-AU ;
    skos:narrower F2021L00304:56 ;
    skos:prefLabel "Item I57"@en-AU ;
    dcat:accessURL <https://www.legislation.gov.au/F2021L00304/asmade/2021-03-24/text/original/epub/OEBPS/document_1/document_1.html#_Toc65844063> ;
    dcat:landingPage "https://www.legislation.gov.au/F2021L00304/asmade/2021-03-24/text/original/epub/OEBPS/document_1/document_1.html#_Toc65844063"^^xsd:anyURI ;
    dcat:theme legcons:Item .

F2021L00304:58 a legcons:Item,
        owl:Class,
        dcat:Resource ;
    rdfs:label "Item - I58 4 18  Other grounds for suspension"@en-AU ;
    dct:isPartOf F2021L00304:56 ;
    dct:isReferencedBy F2021L00304: ;
    rdfs:comment "4 18  Other grounds for suspension - Abrievated Graph Key: I58"@en-AU ;
    skos:definition "4 18  Other grounds for suspension"@en-AU ;
    skos:narrower F2021L00304:56 ;
    skos:prefLabel "Item I58"@en-AU ;
    dcat:accessURL <https://www.legislation.gov.au/F2021L00304/asmade/2021-03-24/text/original/epub/OEBPS/document_1/document_1.html#_Toc65844064> ;
    dcat:landingPage "https://www.legislation.gov.au/F2021L00304/asmade/2021-03-24/text/original/epub/OEBPS/document_1/document_1.html#_Toc65844064"^^xsd:anyURI ;
    dcat:theme legcons:Item .

F2021L00304:6 a legcons:Item,
        owl:Class,
        dcat:Resource ;
    rdfs:label "Item - I6 1 4  Simplified outline of this instrument"@en-AU ;
    dct:isPartOf F2021L00304:1 ;
    dct:isReferencedBy F2021L00304: ;
    rdfs:comment "1 4  Simplified outline of this instrument - Abrievated Graph Key: I6"@en-AU ;
    skos:definition "1 4  Simplified outline of this instrument"@en-AU ;
    skos:narrower F2021L00304:1 ;
    skos:prefLabel "Item I6"@en-AU ;
    dcat:accessURL <https://www.legislation.gov.au/F2021L00304/asmade/2021-03-24/text/original/epub/OEBPS/document_1/document_1.html#_Toc65844012> ;
    dcat:landingPage "https://www.legislation.gov.au/F2021L00304/asmade/2021-03-24/text/original/epub/OEBPS/document_1/document_1.html#_Toc65844012"^^xsd:anyURI ;
    dcat:theme legcons:Item .

F2021L00304:60 a legcons:Item,
        owl:Class,
        dcat:Resource ;
    rdfs:label "Item - I60 4 19  Application of this Part"@en-AU ;
    dct:isPartOf F2021L00304:59 ;
    dct:isReferencedBy F2021L00304: ;
    rdfs:comment "4 19  Application of this Part - Abrievated Graph Key: I60"@en-AU ;
    skos:definition "4 19  Application of this Part"@en-AU ;
    skos:narrower F2021L00304:59 ;
    skos:prefLabel "Item I60"@en-AU ;
    dcat:accessURL <https://www.legislation.gov.au/F2021L00304/asmade/2021-03-24/text/original/epub/OEBPS/document_1/document_1.html#_Toc65844066> ;
    dcat:landingPage "https://www.legislation.gov.au/F2021L00304/asmade/2021-03-24/text/original/epub/OEBPS/document_1/document_1.html#_Toc65844066"^^xsd:anyURI ;
    dcat:theme legcons:Item .

F2021L00304:61 a legcons:Item,
        owl:Class,
        dcat:Resource ;
    rdfs:label "Item - I61 4 20  Initial consideration period"@en-AU ;
    dct:isPartOf F2021L00304:59 ;
    dct:isReferencedBy F2021L00304: ;
    rdfs:comment "4 20  Initial consideration period - Abrievated Graph Key: I61"@en-AU ;
    skos:definition "4 20  Initial consideration period"@en-AU ;
    skos:narrower F2021L00304:59 ;
    skos:prefLabel "Item I61"@en-AU ;
    dcat:accessURL <https://www.legislation.gov.au/F2021L00304/asmade/2021-03-24/text/original/epub/OEBPS/document_1/document_1.html#_Toc65844067> ;
    dcat:landingPage "https://www.legislation.gov.au/F2021L00304/asmade/2021-03-24/text/original/epub/OEBPS/document_1/document_1.html#_Toc65844067"^^xsd:anyURI ;
    dcat:theme legcons:Item .

F2021L00304:62 a legcons:Item,
        owl:Class,
        dcat:Resource ;
    rdfs:label "Item - I62 4 21  Period within which request relating to application must be complied with"@en-AU ;
    dct:isPartOf F2021L00304:59 ;
    dct:isReferencedBy F2021L00304: ;
    rdfs:comment "4 21  Period within which request relating to application must be complied with - Abrievated Graph Key: I62"@en-AU ;
    skos:definition "4 21  Period within which request relating to application must be complied with"@en-AU ;
    skos:narrower F2021L00304:59 ;
    skos:prefLabel "Item I62"@en-AU ;
    dcat:accessURL <https://www.legislation.gov.au/F2021L00304/asmade/2021-03-24/text/original/epub/OEBPS/document_1/document_1.html#_Toc65844068> ;
    dcat:landingPage "https://www.legislation.gov.au/F2021L00304/asmade/2021-03-24/text/original/epub/OEBPS/document_1/document_1.html#_Toc65844068"^^xsd:anyURI ;
    dcat:theme legcons:Item .

F2021L00304:65 a legcons:Item,
        owl:Class,
        dcat:Resource ;
    rdfs:label "Item - I65 5 1  Purpose of this Part"@en-AU ;
    dct:isPartOf F2021L00304:64 ;
    dct:isReferencedBy F2021L00304: ;
    rdfs:comment "5 1  Purpose of this Part - Abrievated Graph Key: I65"@en-AU ;
    skos:definition "5 1  Purpose of this Part"@en-AU ;
    skos:narrower F2021L00304:64 ;
    skos:prefLabel "Item I65"@en-AU ;
    dcat:accessURL <https://www.legislation.gov.au/F2021L00304/asmade/2021-03-24/text/original/epub/OEBPS/document_1/document_1.html#_Toc65844071> ;
    dcat:landingPage "https://www.legislation.gov.au/F2021L00304/asmade/2021-03-24/text/original/epub/OEBPS/document_1/document_1.html#_Toc65844071"^^xsd:anyURI ;
    dcat:theme legcons:Item .

F2021L00304:66 a legcons:Item,
        owl:Class,
        dcat:Resource ;
    rdfs:label "Item - I66 5 2  Proposed arrangement for operations to prepare prescribed milk or milk products"@en-AU ;
    dct:isPartOf F2021L00304:64 ;
    dct:isReferencedBy F2021L00304: ;
    rdfs:comment "5 2  Proposed arrangement for operations to prepare prescribed milk or milk products - Abrievated Graph Key: I66"@en-AU ;
    skos:definition "5 2  Proposed arrangement for operations to prepare prescribed milk or milk products"@en-AU ;
    skos:narrower F2021L00304:64 ;
    skos:prefLabel "Item I66"@en-AU ;
    dcat:accessURL <https://www.legislation.gov.au/F2021L00304/asmade/2021-03-24/text/original/epub/OEBPS/document_1/document_1.html#_Toc65844072> ;
    dcat:landingPage "https://www.legislation.gov.au/F2021L00304/asmade/2021-03-24/text/original/epub/OEBPS/document_1/document_1.html#_Toc65844072"^^xsd:anyURI ;
    dcat:theme legcons:Item .

F2021L00304:67 a legcons:Item,
        owl:Class,
        dcat:Resource ;
    rdfs:label "Item - I67 5 3  Equipment"@en-AU ;
    dct:isPartOf F2021L00304:64 ;
    dct:isReferencedBy F2021L00304: ;
    rdfs:comment "5 3  Equipment - Abrievated Graph Key: I67"@en-AU ;
    skos:definition "5 3  Equipment"@en-AU ;
    skos:narrower F2021L00304:64 ;
    skos:prefLabel "Item I67"@en-AU ;
    dcat:accessURL <https://www.legislation.gov.au/F2021L00304/asmade/2021-03-24/text/original/epub/OEBPS/document_1/document_1.html#_Toc65844073> ;
    dcat:landingPage "https://www.legislation.gov.au/F2021L00304/asmade/2021-03-24/text/original/epub/OEBPS/document_1/document_1.html#_Toc65844073"^^xsd:anyURI ;
    dcat:theme legcons:Item .

F2021L00304:68 a legcons:Item,
        owl:Class,
        dcat:Resource ;
    rdfs:label "Item - I68 5 4  Operational hygiene"@en-AU ;
    dct:isPartOf F2021L00304:64 ;
    dct:isReferencedBy F2021L00304: ;
    rdfs:comment "5 4  Operational hygiene - Abrievated Graph Key: I68"@en-AU ;
    skos:definition "5 4  Operational hygiene"@en-AU ;
    skos:narrower F2021L00304:64 ;
    skos:prefLabel "Item I68"@en-AU ;
    dcat:accessURL <https://www.legislation.gov.au/F2021L00304/asmade/2021-03-24/text/original/epub/OEBPS/document_1/document_1.html#_Toc65844074> ;
    dcat:landingPage "https://www.legislation.gov.au/F2021L00304/asmade/2021-03-24/text/original/epub/OEBPS/document_1/document_1.html#_Toc65844074"^^xsd:anyURI ;
    dcat:theme legcons:Item .

F2021L00304:69 a legcons:Item,
        owl:Class,
        dcat:Resource ;
    rdfs:label "Item - I69 5 5  Identification traceability and integrity"@en-AU ;
    dct:isPartOf F2021L00304:64 ;
    dct:isReferencedBy F2021L00304: ;
    rdfs:comment "5 5  Identification traceability and integrity - Abrievated Graph Key: I69"@en-AU ;
    skos:definition "5 5  Identification traceability and integrity"@en-AU ;
    skos:narrower F2021L00304:64 ;
    skos:prefLabel "Item I69"@en-AU ;
    dcat:accessURL <https://www.legislation.gov.au/F2021L00304/asmade/2021-03-24/text/original/epub/OEBPS/document_1/document_1.html#_Toc65844075> ;
    dcat:landingPage "https://www.legislation.gov.au/F2021L00304/asmade/2021-03-24/text/original/epub/OEBPS/document_1/document_1.html#_Toc65844075"^^xsd:anyURI ;
    dcat:theme legcons:Item .

F2021L00304:7 a legcons:Part,
        owl:Class,
        dcat:Resource ;
    rdfs:label "Part - P7 Part 2 Interpretation"@en-AU ;
    dct:isPartOf F2021L00304:1 ;
    dct:isReferencedBy F2021L00304: ;
    rdfs:comment "Part 2 Interpretation - Abrievated Graph Key: P7"@en-AU ;
    skos:definition "Part 2 Interpretation"@en-AU ;
    skos:narrower F2021L00304:1 ;
    skos:prefLabel "Part P7"@en-AU ;
    dcat:accessURL <https://www.legislation.gov.au/F2021L00304/asmade/2021-03-24/text/original/epub/OEBPS/document_1/document_1.html#_Toc65844013> ;
    dcat:landingPage "https://www.legislation.gov.au/F2021L00304/asmade/2021-03-24/text/original/epub/OEBPS/document_1/document_1.html#_Toc65844013"^^xsd:anyURI ;
    dcat:theme legcons:Part .

F2021L00304:72 a legcons:Item,
        owl:Class,
        dcat:Resource ;
    rdfs:label "Item - I72 5 6  Purpose of this Part"@en-AU ;
    dct:isPartOf F2021L00304:71 ;
    dct:isReferencedBy F2021L00304: ;
    rdfs:comment "5 6  Purpose of this Part - Abrievated Graph Key: I72"@en-AU ;
    skos:definition "5 6  Purpose of this Part"@en-AU ;
    skos:narrower F2021L00304:71 ;
    skos:prefLabel "Item I72"@en-AU ;
    dcat:accessURL <https://www.legislation.gov.au/F2021L00304/asmade/2021-03-24/text/original/epub/OEBPS/document_1/document_1.html#_Toc65844078> ;
    dcat:landingPage "https://www.legislation.gov.au/F2021L00304/asmade/2021-03-24/text/original/epub/OEBPS/document_1/document_1.html#_Toc65844078"^^xsd:anyURI ;
    dcat:theme legcons:Item .

F2021L00304:74 a legcons:Item,
        owl:Class,
        dcat:Resource ;
    rdfs:label "Item - I74 5 7  Importing country requirements must be met"@en-AU ;
    dct:isPartOf F2021L00304:73 ;
    dct:isReferencedBy F2021L00304: ;
    rdfs:comment "5 7  Importing country requirements must be met - Abrievated Graph Key: I74"@en-AU ;
    skos:definition "5 7  Importing country requirements must be met"@en-AU ;
    skos:narrower F2021L00304:73 ;
    skos:prefLabel "Item I74"@en-AU ;
    dcat:accessURL <https://www.legislation.gov.au/F2021L00304/asmade/2021-03-24/text/original/epub/OEBPS/document_1/document_1.html#_Toc65844080> ;
    dcat:landingPage "https://www.legislation.gov.au/F2021L00304/asmade/2021-03-24/text/original/epub/OEBPS/document_1/document_1.html#_Toc65844080"^^xsd:anyURI ;
    dcat:theme legcons:Item .

F2021L00304:76 a legcons:Item,
        owl:Class,
        dcat:Resource ;
    rdfs:label "Item - I76 5 8  Purpose of this Division"@en-AU ;
    dct:isPartOf F2021L00304:75 ;
    dct:isReferencedBy F2021L00304: ;
    rdfs:comment "5 8  Purpose of this Division - Abrievated Graph Key: I76"@en-AU ;
    skos:definition "5 8  Purpose of this Division"@en-AU ;
    skos:narrower F2021L00304:75 ;
    skos:prefLabel "Item I76"@en-AU ;
    dcat:accessURL <https://www.legislation.gov.au/F2021L00304/asmade/2021-03-24/text/original/epub/OEBPS/document_1/document_1.html#_Toc65844082> ;
    dcat:landingPage "https://www.legislation.gov.au/F2021L00304/asmade/2021-03-24/text/original/epub/OEBPS/document_1/document_1.html#_Toc65844082"^^xsd:anyURI ;
    dcat:theme legcons:Item .

F2021L00304:77 a legcons:Item,
        owl:Class,
        dcat:Resource ;
    rdfs:label "Item - I77 5 9  Hygiene controlestablishment and its equipment"@en-AU ;
    dct:isPartOf F2021L00304:75 ;
    dct:isReferencedBy F2021L00304: ;
    rdfs:comment "5 9  Hygiene controlestablishment and its equipment - Abrievated Graph Key: I77"@en-AU ;
    skos:definition "5 9  Hygiene controlestablishment and its equipment"@en-AU ;
    skos:narrower F2021L00304:75 ;
    skos:prefLabel "Item I77"@en-AU ;
    dcat:accessURL <https://www.legislation.gov.au/F2021L00304/asmade/2021-03-24/text/original/epub/OEBPS/document_1/document_1.html#_Toc65844083> ;
    dcat:landingPage "https://www.legislation.gov.au/F2021L00304/asmade/2021-03-24/text/original/epub/OEBPS/document_1/document_1.html#_Toc65844083"^^xsd:anyURI ;
    dcat:theme legcons:Item .

F2021L00304:78 a legcons:Item,
        owl:Class,
        dcat:Resource ;
    rdfs:label "Item - I78 5 10  Measuring devices"@en-AU ;
    dct:isPartOf F2021L00304:75 ;
    dct:isReferencedBy F2021L00304: ;
    rdfs:comment "5 10  Measuring devices - Abrievated Graph Key: I78"@en-AU ;
    skos:definition "5 10  Measuring devices"@en-AU ;
    skos:narrower F2021L00304:75 ;
    skos:prefLabel "Item I78"@en-AU ;
    dcat:accessURL <https://www.legislation.gov.au/F2021L00304/asmade/2021-03-24/text/original/epub/OEBPS/document_1/document_1.html#_Toc65844084> ;
    dcat:landingPage "https://www.legislation.gov.au/F2021L00304/asmade/2021-03-24/text/original/epub/OEBPS/document_1/document_1.html#_Toc65844084"^^xsd:anyURI ;
    dcat:theme legcons:Item .

F2021L00304:79 a legcons:Item,
        owl:Class,
        dcat:Resource ;
    rdfs:label "Item - I79 5 11  Hygiene controlprocessing"@en-AU ;
    dct:isPartOf F2021L00304:75 ;
    dct:isReferencedBy F2021L00304: ;
    rdfs:comment "5 11  Hygiene controlprocessing - Abrievated Graph Key: I79"@en-AU ;
    skos:definition "5 11  Hygiene controlprocessing"@en-AU ;
    skos:narrower F2021L00304:75 ;
    skos:prefLabel "Item I79"@en-AU ;
    dcat:accessURL <https://www.legislation.gov.au/F2021L00304/asmade/2021-03-24/text/original/epub/OEBPS/document_1/document_1.html#_Toc65844085> ;
    dcat:landingPage "https://www.legislation.gov.au/F2021L00304/asmade/2021-03-24/text/original/epub/OEBPS/document_1/document_1.html#_Toc65844085"^^xsd:anyURI ;
    dcat:theme legcons:Item .

F2021L00304:8 a legcons:Item,
        owl:Class,
        dcat:Resource ;
    rdfs:label "Item - I8 1 5  Definitions"@en-AU ;
    dct:isPartOf F2021L00304:1 ;
    dct:isReferencedBy F2021L00304: ;
    rdfs:comment "1 5  Definitions - Abrievated Graph Key: I8"@en-AU ;
    skos:definition "1 5  Definitions"@en-AU ;
    skos:narrower F2021L00304:1 ;
    skos:prefLabel "Item I8"@en-AU ;
    dcat:accessURL <https://www.legislation.gov.au/F2021L00304/asmade/2021-03-24/text/original/epub/OEBPS/document_1/document_1.html#_Toc65844014> ;
    dcat:landingPage "https://www.legislation.gov.au/F2021L00304/asmade/2021-03-24/text/original/epub/OEBPS/document_1/document_1.html#_Toc65844014"^^xsd:anyURI ;
    dcat:theme legcons:Item .

F2021L00304:80 a legcons:Item,
        owl:Class,
        dcat:Resource ;
    rdfs:label "Item - I80 5 12  Personal hygiene and health"@en-AU ;
    dct:isPartOf F2021L00304:75 ;
    dct:isReferencedBy F2021L00304: ;
    rdfs:comment "5 12  Personal hygiene and health - Abrievated Graph Key: I80"@en-AU ;
    skos:definition "5 12  Personal hygiene and health"@en-AU ;
    skos:narrower F2021L00304:75 ;
    skos:prefLabel "Item I80"@en-AU ;
    dcat:accessURL <https://www.legislation.gov.au/F2021L00304/asmade/2021-03-24/text/original/epub/OEBPS/document_1/document_1.html#_Toc65844086> ;
    dcat:landingPage "https://www.legislation.gov.au/F2021L00304/asmade/2021-03-24/text/original/epub/OEBPS/document_1/document_1.html#_Toc65844086"^^xsd:anyURI ;
    dcat:theme legcons:Item .

F2021L00304:82 a legcons:Item,
        owl:Class,
        dcat:Resource ;
    rdfs:label "Item - I82 5 13  Sourcing milk and milk products"@en-AU ;
    dct:isPartOf F2021L00304:81 ;
    dct:isReferencedBy F2021L00304: ;
    rdfs:comment "5 13  Sourcing milk and milk products - Abrievated Graph Key: I82"@en-AU ;
    skos:definition "5 13  Sourcing milk and milk products"@en-AU ;
    skos:narrower F2021L00304:81 ;
    skos:prefLabel "Item I82"@en-AU ;
    dcat:accessURL <https://www.legislation.gov.au/F2021L00304/asmade/2021-03-24/text/original/epub/OEBPS/document_1/document_1.html#_Toc65844088> ;
    dcat:landingPage "https://www.legislation.gov.au/F2021L00304/asmade/2021-03-24/text/original/epub/OEBPS/document_1/document_1.html#_Toc65844088"^^xsd:anyURI ;
    dcat:theme legcons:Item .

F2021L00304:83 a legcons:Item,
        owl:Class,
        dcat:Resource ;
    rdfs:label "Item - I83 5 14  Notifiable diseases"@en-AU ;
    dct:isPartOf F2021L00304:81 ;
    dct:isReferencedBy F2021L00304: ;
    rdfs:comment "5 14  Notifiable diseases - Abrievated Graph Key: I83"@en-AU ;
    skos:definition "5 14  Notifiable diseases"@en-AU ;
    skos:narrower F2021L00304:81 ;
    skos:prefLabel "Item I83"@en-AU ;
    dcat:accessURL <https://www.legislation.gov.au/F2021L00304/asmade/2021-03-24/text/original/epub/OEBPS/document_1/document_1.html#_Toc65844089> ;
    dcat:landingPage "https://www.legislation.gov.au/F2021L00304/asmade/2021-03-24/text/original/epub/OEBPS/document_1/document_1.html#_Toc65844089"^^xsd:anyURI ;
    dcat:theme legcons:Item .

F2021L00304:84 a legcons:Item,
        owl:Class,
        dcat:Resource ;
    rdfs:label "Item - I84 5 15  Temperature controls for preparing prescribed milk or milk products"@en-AU ;
    dct:isPartOf F2021L00304:81 ;
    dct:isReferencedBy F2021L00304: ;
    rdfs:comment "5 15  Temperature controls for preparing prescribed milk or milk products - Abrievated Graph Key: I84"@en-AU ;
    skos:definition "5 15  Temperature controls for preparing prescribed milk or milk products"@en-AU ;
    skos:narrower F2021L00304:81 ;
    skos:prefLabel "Item I84"@en-AU ;
    dcat:accessURL <https://www.legislation.gov.au/F2021L00304/asmade/2021-03-24/text/original/epub/OEBPS/document_1/document_1.html#_Toc65844090> ;
    dcat:landingPage "https://www.legislation.gov.au/F2021L00304/asmade/2021-03-24/text/original/epub/OEBPS/document_1/document_1.html#_Toc65844090"^^xsd:anyURI ;
    dcat:theme legcons:Item .

F2021L00304:85 a legcons:Item,
        owl:Class,
        dcat:Resource ;
    rdfs:label "Item - I85 5 16  Temperature controls for storing handling loading and transporting prescribed milk or milk products"@en-AU ;
    dct:isPartOf F2021L00304:81 ;
    dct:isReferencedBy F2021L00304: ;
    rdfs:comment "5 16  Temperature controls for storing handling loading and transporting prescribed milk or milk products - Abrievated Graph Key: I85"@en-AU ;
    skos:definition "5 16  Temperature controls for storing handling loading and transporting prescribed milk or milk products"@en-AU ;
    skos:narrower F2021L00304:81 ;
    skos:prefLabel "Item I85"@en-AU ;
    dcat:accessURL <https://www.legislation.gov.au/F2021L00304/asmade/2021-03-24/text/original/epub/OEBPS/document_1/document_1.html#_Toc65844091> ;
    dcat:landingPage "https://www.legislation.gov.au/F2021L00304/asmade/2021-03-24/text/original/epub/OEBPS/document_1/document_1.html#_Toc65844091"^^xsd:anyURI ;
    dcat:theme legcons:Item .

F2021L00304:86 a legcons:Item,
        owl:Class,
        dcat:Resource ;
    rdfs:label "Item - I86 5 17  Preserving prescribed milk and milk products"@en-AU ;
    dct:isPartOf F2021L00304:81 ;
    dct:isReferencedBy F2021L00304: ;
    rdfs:comment "5 17  Preserving prescribed milk and milk products - Abrievated Graph Key: I86"@en-AU ;
    skos:definition "5 17  Preserving prescribed milk and milk products"@en-AU ;
    skos:narrower F2021L00304:81 ;
    skos:prefLabel "Item I86"@en-AU ;
    dcat:accessURL <https://www.legislation.gov.au/F2021L00304/asmade/2021-03-24/text/original/epub/OEBPS/document_1/document_1.html#_Toc65844092> ;
    dcat:landingPage "https://www.legislation.gov.au/F2021L00304/asmade/2021-03-24/text/original/epub/OEBPS/document_1/document_1.html#_Toc65844092"^^xsd:anyURI ;
    dcat:theme legcons:Item .

F2021L00304:87 a legcons:Item,
        owl:Class,
        dcat:Resource ;
    rdfs:label "Item - I87 5 18  Thermal processing of canned prescribed milk or milk products"@en-AU ;
    dct:isPartOf F2021L00304:81 ;
    dct:isReferencedBy F2021L00304: ;
    rdfs:comment "5 18  Thermal processing of canned prescribed milk or milk products - Abrievated Graph Key: I87"@en-AU ;
    skos:definition "5 18  Thermal processing of canned prescribed milk or milk products"@en-AU ;
    skos:narrower F2021L00304:81 ;
    skos:prefLabel "Item I87"@en-AU ;
    dcat:accessURL <https://www.legislation.gov.au/F2021L00304/asmade/2021-03-24/text/original/epub/OEBPS/document_1/document_1.html#_Toc65844093> ;
    dcat:landingPage "https://www.legislation.gov.au/F2021L00304/asmade/2021-03-24/text/original/epub/OEBPS/document_1/document_1.html#_Toc65844093"^^xsd:anyURI ;
    dcat:theme legcons:Item .

F2021L00304:88 a legcons:Item,
        owl:Class,
        dcat:Resource ;
    rdfs:label "Item - I88 5 19  Pasteurisation and other treatments"@en-AU ;
    dct:isPartOf F2021L00304:81 ;
    dct:isReferencedBy F2021L00304: ;
    rdfs:comment "5 19  Pasteurisation and other treatments - Abrievated Graph Key: I88"@en-AU ;
    skos:definition "5 19  Pasteurisation and other treatments"@en-AU ;
    skos:narrower F2021L00304:81 ;
    skos:prefLabel "Item I88"@en-AU ;
    dcat:accessURL <https://www.legislation.gov.au/F2021L00304/asmade/2021-03-24/text/original/epub/OEBPS/document_1/document_1.html#_Toc65844094> ;
    dcat:landingPage "https://www.legislation.gov.au/F2021L00304/asmade/2021-03-24/text/original/epub/OEBPS/document_1/document_1.html#_Toc65844094"^^xsd:anyURI ;
    dcat:theme legcons:Item .

F2021L00304:89 a legcons:Item,
        owl:Class,
        dcat:Resource ;
    rdfs:label "Item - I89 5 20  Packaging and identification"@en-AU ;
    dct:isPartOf F2021L00304:81 ;
    dct:isReferencedBy F2021L00304: ;
    rdfs:comment "5 20  Packaging and identification - Abrievated Graph Key: I89"@en-AU ;
    skos:definition "5 20  Packaging and identification"@en-AU ;
    skos:narrower F2021L00304:81 ;
    skos:prefLabel "Item I89"@en-AU ;
    dcat:accessURL <https://www.legislation.gov.au/F2021L00304/asmade/2021-03-24/text/original/epub/OEBPS/document_1/document_1.html#_Toc65844095> ;
    dcat:landingPage "https://www.legislation.gov.au/F2021L00304/asmade/2021-03-24/text/original/epub/OEBPS/document_1/document_1.html#_Toc65844095"^^xsd:anyURI ;
    dcat:theme legcons:Item .

F2021L00304:9 a legcons:Item,
        owl:Class,
        dcat:Resource ;
    rdfs:label "Item - I9 1 6  Meaning of loaded for export"@en-AU ;
    dct:isPartOf F2021L00304:1 ;
    dct:isReferencedBy F2021L00304: ;
    rdfs:comment "1 6  Meaning of loaded for export - Abrievated Graph Key: I9"@en-AU ;
    skos:definition "1 6  Meaning of loaded for export"@en-AU ;
    skos:narrower F2021L00304:1 ;
    skos:prefLabel "Item I9"@en-AU ;
    dcat:accessURL <https://www.legislation.gov.au/F2021L00304/asmade/2021-03-24/text/original/epub/OEBPS/document_1/document_1.html#_Toc65844015> ;
    dcat:landingPage "https://www.legislation.gov.au/F2021L00304/asmade/2021-03-24/text/original/epub/OEBPS/document_1/document_1.html#_Toc65844015"^^xsd:anyURI ;
    dcat:theme legcons:Item .

F2021L00304:90 a legcons:Item,
        owl:Class,
        dcat:Resource ;
    rdfs:label "Item - I90 5 21  Storage handling and loading"@en-AU ;
    dct:isPartOf F2021L00304:81 ;
    dct:isReferencedBy F2021L00304: ;
    rdfs:comment "5 21  Storage handling and loading - Abrievated Graph Key: I90"@en-AU ;
    skos:definition "5 21  Storage handling and loading"@en-AU ;
    skos:narrower F2021L00304:81 ;
    skos:prefLabel "Item I90"@en-AU ;
    dcat:accessURL <https://www.legislation.gov.au/F2021L00304/asmade/2021-03-24/text/original/epub/OEBPS/document_1/document_1.html#_Toc65844096> ;
    dcat:landingPage "https://www.legislation.gov.au/F2021L00304/asmade/2021-03-24/text/original/epub/OEBPS/document_1/document_1.html#_Toc65844096"^^xsd:anyURI ;
    dcat:theme legcons:Item .

F2021L00304:91 a legcons:Item,
        owl:Class,
        dcat:Resource ;
    rdfs:label "Item - I91 5 22  Container system units and food carrying compartments of vehiclesconstruction etc"@en-AU ;
    dct:isPartOf F2021L00304:81 ;
    dct:isReferencedBy F2021L00304: ;
    rdfs:comment "5 22  Container system units and food carrying compartments of vehiclesconstruction etc - Abrievated Graph Key: I91"@en-AU ;
    skos:definition "5 22  Container system units and food carrying compartments of vehiclesconstruction etc"@en-AU ;
    skos:narrower F2021L00304:81 ;
    skos:prefLabel "Item I91"@en-AU ;
    dcat:accessURL <https://www.legislation.gov.au/F2021L00304/asmade/2021-03-24/text/original/epub/OEBPS/document_1/document_1.html#_Toc65844097> ;
    dcat:landingPage "https://www.legislation.gov.au/F2021L00304/asmade/2021-03-24/text/original/epub/OEBPS/document_1/document_1.html#_Toc65844097"^^xsd:anyURI ;
    dcat:theme legcons:Item .

F2021L00304:92 a legcons:Item,
        owl:Class,
        dcat:Resource ;
    rdfs:label "Item - I92 5 23  Vehicles container system units etchygiene control"@en-AU ;
    dct:isPartOf F2021L00304:81 ;
    dct:isReferencedBy F2021L00304: ;
    rdfs:comment "5 23  Vehicles container system units etchygiene control - Abrievated Graph Key: I92"@en-AU ;
    skos:definition "5 23  Vehicles container system units etchygiene control"@en-AU ;
    skos:narrower F2021L00304:81 ;
    skos:prefLabel "Item I92"@en-AU ;
    dcat:accessURL <https://www.legislation.gov.au/F2021L00304/asmade/2021-03-24/text/original/epub/OEBPS/document_1/document_1.html#_Toc65844098> ;
    dcat:landingPage "https://www.legislation.gov.au/F2021L00304/asmade/2021-03-24/text/original/epub/OEBPS/document_1/document_1.html#_Toc65844098"^^xsd:anyURI ;
    dcat:theme legcons:Item .

F2021L00304:93 a legcons:Item,
        owl:Class,
        dcat:Resource ;
    rdfs:label "Item - I93 5 24  Transport"@en-AU ;
    dct:isPartOf F2021L00304:81 ;
    dct:isReferencedBy F2021L00304: ;
    rdfs:comment "5 24  Transport - Abrievated Graph Key: I93"@en-AU ;
    skos:definition "5 24  Transport"@en-AU ;
    skos:narrower F2021L00304:81 ;
    skos:prefLabel "Item I93"@en-AU ;
    dcat:accessURL <https://www.legislation.gov.au/F2021L00304/asmade/2021-03-24/text/original/epub/OEBPS/document_1/document_1.html#_Toc65844099> ;
    dcat:landingPage "https://www.legislation.gov.au/F2021L00304/asmade/2021-03-24/text/original/epub/OEBPS/document_1/document_1.html#_Toc65844099"^^xsd:anyURI ;
    dcat:theme legcons:Item .

F2021L00304:94 a legcons:Item,
        owl:Class,
        dcat:Resource ;
    rdfs:label "Item - I94 5 25  Identification as not for export as foodfitness for human consumption etc"@en-AU ;
    dct:isPartOf F2021L00304:81 ;
    dct:isReferencedBy F2021L00304: ;
    rdfs:comment "5 25  Identification as not for export as foodfitness for human consumption etc - Abrievated Graph Key: I94"@en-AU ;
    skos:definition "5 25  Identification as not for export as foodfitness for human consumption etc"@en-AU ;
    skos:narrower F2021L00304:81 ;
    skos:prefLabel "Item I94"@en-AU ;
    dcat:accessURL <https://www.legislation.gov.au/F2021L00304/asmade/2021-03-24/text/original/epub/OEBPS/document_1/document_1.html#_Toc65844100> ;
    dcat:landingPage "https://www.legislation.gov.au/F2021L00304/asmade/2021-03-24/text/original/epub/OEBPS/document_1/document_1.html#_Toc65844100"^^xsd:anyURI ;
    dcat:theme legcons:Item .

F2021L00304:95 a legcons:Item,
        owl:Class,
        dcat:Resource ;
    rdfs:label "Item - I95 5 26  Product standardsgeneral"@en-AU ;
    dct:isPartOf F2021L00304:81 ;
    dct:isReferencedBy F2021L00304: ;
    rdfs:comment "5 26  Product standardsgeneral - Abrievated Graph Key: I95"@en-AU ;
    skos:definition "5 26  Product standardsgeneral"@en-AU ;
    skos:narrower F2021L00304:81 ;
    skos:prefLabel "Item I95"@en-AU ;
    dcat:accessURL <https://www.legislation.gov.au/F2021L00304/asmade/2021-03-24/text/original/epub/OEBPS/document_1/document_1.html#_Toc65844101> ;
    dcat:landingPage "https://www.legislation.gov.au/F2021L00304/asmade/2021-03-24/text/original/epub/OEBPS/document_1/document_1.html#_Toc65844101"^^xsd:anyURI ;
    dcat:theme legcons:Item .

F2021L00304:97 a legcons:Item,
        owl:Class,
        dcat:Resource ;
    rdfs:label "Item - I97 5 27  Trade description must be applied to prescribed milk and milk products"@en-AU ;
    dct:isPartOf F2021L00304:96 ;
    dct:isReferencedBy F2021L00304: ;
    rdfs:comment "5 27  Trade description must be applied to prescribed milk and milk products - Abrievated Graph Key: I97"@en-AU ;
    skos:definition "5 27  Trade description must be applied to prescribed milk and milk products"@en-AU ;
    skos:narrower F2021L00304:96 ;
    skos:prefLabel "Item I97"@en-AU ;
    dcat:accessURL <https://www.legislation.gov.au/F2021L00304/asmade/2021-03-24/text/original/epub/OEBPS/document_1/document_1.html#_Toc65844103> ;
    dcat:landingPage "https://www.legislation.gov.au/F2021L00304/asmade/2021-03-24/text/original/epub/OEBPS/document_1/document_1.html#_Toc65844103"^^xsd:anyURI ;
    dcat:theme legcons:Item .

F2021L00304:98 a legcons:Item,
        owl:Class,
        dcat:Resource ;
    rdfs:label "Item - I98 5 28  Incomplete trade descriptioncanned milk or milk products"@en-AU ;
    dct:isPartOf F2021L00304:96 ;
    dct:isReferencedBy F2021L00304: ;
    rdfs:comment "5 28  Incomplete trade descriptioncanned milk or milk products - Abrievated Graph Key: I98"@en-AU ;
    skos:definition "5 28  Incomplete trade descriptioncanned milk or milk products"@en-AU ;
    skos:narrower F2021L00304:96 ;
    skos:prefLabel "Item I98"@en-AU ;
    dcat:accessURL <https://www.legislation.gov.au/F2021L00304/asmade/2021-03-24/text/original/epub/OEBPS/document_1/document_1.html#_Toc65844104> ;
    dcat:landingPage "https://www.legislation.gov.au/F2021L00304/asmade/2021-03-24/text/original/epub/OEBPS/document_1/document_1.html#_Toc65844104"^^xsd:anyURI ;
    dcat:theme legcons:Item .

F2021L00304:99 a legcons:Item,
        owl:Class,
        dcat:Resource ;
    rdfs:label "Item - I99 5 29  Labelling and naming of ingredients"@en-AU ;
    dct:isPartOf F2021L00304:96 ;
    dct:isReferencedBy F2021L00304: ;
    rdfs:comment "5 29  Labelling and naming of ingredients - Abrievated Graph Key: I99"@en-AU ;
    skos:definition "5 29  Labelling and naming of ingredients"@en-AU ;
    skos:narrower F2021L00304:96 ;
    skos:prefLabel "Item I99"@en-AU ;
    dcat:accessURL <https://www.legislation.gov.au/F2021L00304/asmade/2021-03-24/text/original/epub/OEBPS/document_1/document_1.html#_Toc65844105> ;
    dcat:landingPage "https://www.legislation.gov.au/F2021L00304/asmade/2021-03-24/text/original/epub/OEBPS/document_1/document_1.html#_Toc65844105"^^xsd:anyURI ;
    dcat:theme legcons:Item .

F2021L00304:101 a legcons:Division,
        owl:Class,
        dcat:Resource ;
    rdfs:label "Division - D101 Division 6 Official marks"@en-AU ;
    dct:hasPart F2021L00304:102 ;
    dct:isPartOf F2021L00304:70 ;
    dct:isReferencedBy F2021L00304: ;
    rdfs:comment "Division 6 Official marks - Abrievated Graph Key: D101"@en-AU ;
    skos:broader F2021L00304:102 ;
    skos:definition "Division 6 Official marks"@en-AU ;
    skos:narrower F2021L00304:70 ;
    skos:prefLabel "Division D101"@en-AU ;
    dcat:accessURL <https://www.legislation.gov.au/F2021L00304/asmade/2021-03-24/text/original/epub/OEBPS/document_1/document_1.html#_Toc65844107> ;
    dcat:landingPage "https://www.legislation.gov.au/F2021L00304/asmade/2021-03-24/text/original/epub/OEBPS/document_1/document_1.html#_Toc65844107"^^xsd:anyURI ;
    dcat:theme legcons:Division .

F2021L00304:116 a legcons:Part,
        owl:Class,
        dcat:Resource ;
    rdfs:label "Part - P116 Part 3 Renewal of approved arrangement"@en-AU ;
    dct:hasPart F2021L00304:117 ;
    dct:isPartOf F2021L00304:63 ;
    dct:isReferencedBy F2021L00304: ;
    rdfs:comment "Part 3 Renewal of approved arrangement - Abrievated Graph Key: P116"@en-AU ;
    skos:broader F2021L00304:117 ;
    skos:definition "Part 3 Renewal of approved arrangement"@en-AU ;
    skos:narrower F2021L00304:63 ;
    skos:prefLabel "Part P116"@en-AU ;
    dcat:accessURL <https://www.legislation.gov.au/F2021L00304/asmade/2021-03-24/text/original/epub/OEBPS/document_1/document_1.html#_Toc65844122> ;
    dcat:landingPage "https://www.legislation.gov.au/F2021L00304/asmade/2021-03-24/text/original/epub/OEBPS/document_1/document_1.html#_Toc65844122"^^xsd:anyURI ;
    dcat:theme legcons:Part .

F2021L00304:122 a legcons:Division,
        owl:Class,
        dcat:Resource ;
    rdfs:label "Division - D122 Division 2 Variations required by Secretary"@en-AU ;
    dct:hasPart F2021L00304:123 ;
    dct:isPartOf F2021L00304:118 ;
    dct:isReferencedBy F2021L00304: ;
    rdfs:comment "Division 2 Variations required by Secretary - Abrievated Graph Key: D122"@en-AU ;
    skos:broader F2021L00304:123 ;
    skos:definition "Division 2 Variations required by Secretary"@en-AU ;
    skos:narrower F2021L00304:118 ;
    skos:prefLabel "Division D122"@en-AU ;
    dcat:accessURL <https://www.legislation.gov.au/F2021L00304/asmade/2021-03-24/text/original/epub/OEBPS/document_1/document_1.html#_Toc65844128> ;
    dcat:landingPage "https://www.legislation.gov.au/F2021L00304/asmade/2021-03-24/text/original/epub/OEBPS/document_1/document_1.html#_Toc65844128"^^xsd:anyURI ;
    dcat:theme legcons:Division .

F2021L00304:143 a legcons:Chapter,
        owl:Class,
        dcat:Resource ;
    rdfs:label "Chapter - C143 Chapter 8 Other matters relating to export"@en-AU ;
    dct:hasPart F2021L00304:144,
        F2021L00304:148 ;
    dct:isReferencedBy F2021L00304: ;
    rdfs:comment "Chapter 8 Other matters relating to export - Abrievated Graph Key: C143"@en-AU ;
    skos:broader F2021L00304:144,
        F2021L00304:148 ;
    skos:definition "Chapter 8 Other matters relating to export"@en-AU ;
    skos:prefLabel "Chapter C143"@en-AU ;
    dcat:accessURL <https://www.legislation.gov.au/F2021L00304/asmade/2021-03-24/text/original/epub/OEBPS/document_1/document_1.html#_Toc65844149> ;
    dcat:landingPage "https://www.legislation.gov.au/F2021L00304/asmade/2021-03-24/text/original/epub/OEBPS/document_1/document_1.html#_Toc65844149"^^xsd:anyURI ;
    dcat:theme legcons:Chapter .

F2021L00304:206 a legcons:Division,
        owl:Class,
        dcat:Resource ;
    rdfs:label "Division - D206 Division 1 General"@en-AU ;
    dct:hasPart F2021L00304:207 ;
    dct:isPartOf F2021L00304:205 ;
    dct:isReferencedBy F2021L00304: ;
    rdfs:comment "Division 1 General - Abrievated Graph Key: D206"@en-AU ;
    skos:broader F2021L00304:207 ;
    skos:definition "Division 1 General"@en-AU ;
    skos:narrower F2021L00304:205 ;
    skos:prefLabel "Division D206"@en-AU ;
    dcat:accessURL <https://www.legislation.gov.au/F2021L00304/asmade/2021-03-24/text/original/epub/OEBPS/document_1/document_1.html#_Toc65844212> ;
    dcat:landingPage "https://www.legislation.gov.au/F2021L00304/asmade/2021-03-24/text/original/epub/OEBPS/document_1/document_1.html#_Toc65844212"^^xsd:anyURI ;
    dcat:theme legcons:Division .

F2021L00304:223 a legcons:Part,
        owl:Class,
        dcat:Resource ;
    rdfs:label "Part - P223 Part 3 Powers of the Secretary"@en-AU ;
    dct:hasPart F2021L00304:224 ;
    dct:isPartOf F2021L00304:183 ;
    dct:isReferencedBy F2021L00304: ;
    rdfs:comment "Part 3 Powers of the Secretary - Abrievated Graph Key: P223"@en-AU ;
    skos:broader F2021L00304:224 ;
    skos:definition "Part 3 Powers of the Secretary"@en-AU ;
    skos:narrower F2021L00304:183 ;
    skos:prefLabel "Part P223"@en-AU ;
    dcat:accessURL <https://www.legislation.gov.au/F2021L00304/asmade/2021-03-24/text/original/epub/OEBPS/document_1/document_1.html#_Toc65844229> ;
    dcat:landingPage "https://www.legislation.gov.au/F2021L00304/asmade/2021-03-24/text/original/epub/OEBPS/document_1/document_1.html#_Toc65844229"^^xsd:anyURI ;
    dcat:theme legcons:Part .

F2021L00304:226 a legcons:Division,
        owl:Class,
        dcat:Resource ;
    rdfs:label "Division - D226 Division 1 Third party authorised officers"@en-AU ;
    dct:hasPart F2021L00304:227 ;
    dct:isPartOf F2021L00304:225 ;
    dct:isReferencedBy F2021L00304: ;
    rdfs:comment "Division 1 Third party authorised officers - Abrievated Graph Key: D226"@en-AU ;
    skos:broader F2021L00304:227 ;
    skos:definition "Division 1 Third party authorised officers"@en-AU ;
    skos:narrower F2021L00304:225 ;
    skos:prefLabel "Division D226"@en-AU ;
    dcat:accessURL <https://www.legislation.gov.au/F2021L00304/asmade/2021-03-24/text/original/epub/OEBPS/document_1/document_1.html#_Toc65844232> ;
    dcat:landingPage "https://www.legislation.gov.au/F2021L00304/asmade/2021-03-24/text/original/epub/OEBPS/document_1/document_1.html#_Toc65844232"^^xsd:anyURI ;
    dcat:theme legcons:Division .

F2021L00304:233 a legcons:Division,
        owl:Class,
        dcat:Resource ;
    rdfs:label "Division - D233 Division 3 Directions to deal with non compliance with the Act etc"@en-AU ;
    dct:hasPart F2021L00304:234 ;
    dct:isPartOf F2021L00304:225 ;
    dct:isReferencedBy F2021L00304: ;
    rdfs:comment "Division 3 Directions to deal with non compliance with the Act etc - Abrievated Graph Key: D233"@en-AU ;
    skos:broader F2021L00304:234 ;
    skos:definition "Division 3 Directions to deal with non compliance with the Act etc"@en-AU ;
    skos:narrower F2021L00304:225 ;
    skos:prefLabel "Division D233"@en-AU ;
    dcat:accessURL <https://www.legislation.gov.au/F2021L00304/asmade/2021-03-24/text/original/epub/OEBPS/document_1/document_1.html#_Toc65844239> ;
    dcat:landingPage "https://www.legislation.gov.au/F2021L00304/asmade/2021-03-24/text/original/epub/OEBPS/document_1/document_1.html#_Toc65844239"^^xsd:anyURI ;
    dcat:theme legcons:Division .

F2021L00304:235 a legcons:Division,
        owl:Class,
        dcat:Resource ;
    rdfs:label "Division - D235 Division 4 Miscellaneous"@en-AU ;
    dct:hasPart F2021L00304:236 ;
    dct:isPartOf F2021L00304:225 ;
    dct:isReferencedBy F2021L00304: ;
    rdfs:comment "Division 4 Miscellaneous - Abrievated Graph Key: D235"@en-AU ;
    skos:broader F2021L00304:236 ;
    skos:definition "Division 4 Miscellaneous"@en-AU ;
    skos:narrower F2021L00304:225 ;
    skos:prefLabel "Division D235"@en-AU ;
    dcat:accessURL <https://www.legislation.gov.au/F2021L00304/asmade/2021-03-24/text/original/epub/OEBPS/document_1/document_1.html#_Toc65844241> ;
    dcat:landingPage "https://www.legislation.gov.au/F2021L00304/asmade/2021-03-24/text/original/epub/OEBPS/document_1/document_1.html#_Toc65844241"^^xsd:anyURI ;
    dcat:theme legcons:Division .

F2021L00304:237 a legcons:Chapter,
        owl:Class,
        dcat:Resource ;
    rdfs:label "Chapter - C237 Chapter 10 Compliance and enforcement"@en-AU ;
    dct:hasPart F2021L00304:238,
        F2021L00304:239 ;
    dct:isReferencedBy F2021L00304: ;
    rdfs:comment "Chapter 10 Compliance and enforcement - Abrievated Graph Key: C237"@en-AU ;
    skos:broader F2021L00304:238,
        F2021L00304:239 ;
    skos:definition "Chapter 10 Compliance and enforcement"@en-AU ;
    skos:prefLabel "Chapter C237"@en-AU ;
    dcat:accessURL <https://www.legislation.gov.au/F2021L00304/asmade/2021-03-24/text/original/epub/OEBPS/document_1/document_1.html#_Toc65844243> ;
    dcat:landingPage "https://www.legislation.gov.au/F2021L00304/asmade/2021-03-24/text/original/epub/OEBPS/document_1/document_1.html#_Toc65844243"^^xsd:anyURI ;
    dcat:theme legcons:Chapter .

F2021L00304:241 a legcons:Part,
        owl:Class,
        dcat:Resource ;
    rdfs:label "Part - P241 Part 1 Review of decisions"@en-AU ;
    dct:hasPart F2021L00304:242 ;
    dct:isPartOf F2021L00304:240 ;
    dct:isReferencedBy F2021L00304: ;
    rdfs:comment "Part 1 Review of decisions - Abrievated Graph Key: P241"@en-AU ;
    skos:broader F2021L00304:242 ;
    skos:definition "Part 1 Review of decisions"@en-AU ;
    skos:narrower F2021L00304:240 ;
    skos:prefLabel "Part P241"@en-AU ;
    dcat:accessURL <https://www.legislation.gov.au/F2021L00304/asmade/2021-03-24/text/original/epub/OEBPS/document_1/document_1.html#_Toc65844247> ;
    dcat:landingPage "https://www.legislation.gov.au/F2021L00304/asmade/2021-03-24/text/original/epub/OEBPS/document_1/document_1.html#_Toc65844247"^^xsd:anyURI ;
    dcat:theme legcons:Part .

F2021L00304:259 a legcons:Part,
        owl:Class,
        dcat:Resource ;
    rdfs:label "Part - P259 Part 5 Relevant Commonwealth liabilities"@en-AU ;
    dct:hasPart F2021L00304:260 ;
    dct:isPartOf F2021L00304:240 ;
    dct:isReferencedBy F2021L00304: ;
    rdfs:comment "Part 5 Relevant Commonwealth liabilities - Abrievated Graph Key: P259"@en-AU ;
    skos:broader F2021L00304:260 ;
    skos:definition "Part 5 Relevant Commonwealth liabilities"@en-AU ;
    skos:narrower F2021L00304:240 ;
    skos:prefLabel "Part P259"@en-AU ;
    dcat:accessURL <https://www.legislation.gov.au/F2021L00304/asmade/2021-03-24/text/original/epub/OEBPS/document_1/document_1.html#_Toc65844265> ;
    dcat:landingPage "https://www.legislation.gov.au/F2021L00304/asmade/2021-03-24/text/original/epub/OEBPS/document_1/document_1.html#_Toc65844265"^^xsd:anyURI ;
    dcat:theme legcons:Part .

F2021L00304:262 a legcons:Part,
        owl:Class,
        dcat:Resource ;
    rdfs:label "Part - P262 Part 1 Preliminary"@en-AU ;
    dct:hasPart F2021L00304:263 ;
    dct:isPartOf F2021L00304:261 ;
    dct:isReferencedBy F2021L00304: ;
    rdfs:comment "Part 1 Preliminary - Abrievated Graph Key: P262"@en-AU ;
    skos:broader F2021L00304:263 ;
    skos:definition "Part 1 Preliminary"@en-AU ;
    skos:narrower F2021L00304:261 ;
    skos:prefLabel "Part P262"@en-AU ;
    dcat:accessURL <https://www.legislation.gov.au/F2021L00304/asmade/2021-03-24/text/original/epub/OEBPS/document_1/document_1.html#_Toc65844268> ;
    dcat:landingPage "https://www.legislation.gov.au/F2021L00304/asmade/2021-03-24/text/original/epub/OEBPS/document_1/document_1.html#_Toc65844268"^^xsd:anyURI ;
    dcat:theme legcons:Part .

F2021L00304:264 a legcons:Part,
        owl:Class,
        dcat:Resource ;
    rdfs:label "Part - P264 Part 2 Approved arrangements"@en-AU ;
    dct:hasPart F2021L00304:265 ;
    dct:isPartOf F2021L00304:261 ;
    dct:isReferencedBy F2021L00304: ;
    rdfs:comment "Part 2 Approved arrangements - Abrievated Graph Key: P264"@en-AU ;
    skos:broader F2021L00304:265 ;
    skos:definition "Part 2 Approved arrangements"@en-AU ;
    skos:narrower F2021L00304:261 ;
    skos:prefLabel "Part P264"@en-AU ;
    dcat:accessURL <https://www.legislation.gov.au/F2021L00304/asmade/2021-03-24/text/original/epub/OEBPS/document_1/document_1.html#_Toc65844270> ;
    dcat:landingPage "https://www.legislation.gov.au/F2021L00304/asmade/2021-03-24/text/original/epub/OEBPS/document_1/document_1.html#_Toc65844270"^^xsd:anyURI ;
    dcat:theme legcons:Part .

F2021L00304:267 a legcons:Division,
        owl:Class,
        dcat:Resource ;
    rdfs:label "Division - D267 Division 1 Trade descriptions"@en-AU ;
    dct:hasPart F2021L00304:268 ;
    dct:isPartOf F2021L00304:266 ;
    dct:isReferencedBy F2021L00304: ;
    rdfs:comment "Division 1 Trade descriptions - Abrievated Graph Key: D267"@en-AU ;
    skos:broader F2021L00304:268 ;
    skos:definition "Division 1 Trade descriptions"@en-AU ;
    skos:narrower F2021L00304:266 ;
    skos:prefLabel "Division D267"@en-AU ;
    dcat:accessURL <https://www.legislation.gov.au/F2021L00304/asmade/2021-03-24/text/original/epub/OEBPS/document_1/document_1.html#_Toc65844273> ;
    dcat:landingPage "https://www.legislation.gov.au/F2021L00304/asmade/2021-03-24/text/original/epub/OEBPS/document_1/document_1.html#_Toc65844273"^^xsd:anyURI ;
    dcat:theme legcons:Division .

F2021L00304:281 a legcons:Division,
        owl:Class,
        dcat:Resource ;
    rdfs:label "Division - D281 Division 2 Assessments"@en-AU ;
    dct:hasPart F2021L00304:282 ;
    dct:isPartOf F2021L00304:276 ;
    dct:isReferencedBy F2021L00304: ;
    rdfs:comment "Division 2 Assessments - Abrievated Graph Key: D281"@en-AU ;
    skos:broader F2021L00304:282 ;
    skos:definition "Division 2 Assessments"@en-AU ;
    skos:narrower F2021L00304:276 ;
    skos:prefLabel "Division D281"@en-AU ;
    dcat:accessURL <https://www.legislation.gov.au/F2021L00304/asmade/2021-03-24/text/original/epub/OEBPS/document_1/document_1.html#_Toc65844287> ;
    dcat:landingPage "https://www.legislation.gov.au/F2021L00304/asmade/2021-03-24/text/original/epub/OEBPS/document_1/document_1.html#_Toc65844287"^^xsd:anyURI ;
    dcat:theme legcons:Division .

F2021L00304:71 a legcons:Division,
        owl:Class,
        dcat:Resource ;
    rdfs:label "Division - D71 Division 1 Purpose of this Part"@en-AU ;
    dct:hasPart F2021L00304:72 ;
    dct:isPartOf F2021L00304:70 ;
    dct:isReferencedBy F2021L00304: ;
    rdfs:comment "Division 1 Purpose of this Part - Abrievated Graph Key: D71"@en-AU ;
    skos:broader F2021L00304:72 ;
    skos:definition "Division 1 Purpose of this Part"@en-AU ;
    skos:narrower F2021L00304:70 ;
    skos:prefLabel "Division D71"@en-AU ;
    dcat:accessURL <https://www.legislation.gov.au/F2021L00304/asmade/2021-03-24/text/original/epub/OEBPS/document_1/document_1.html#_Toc65844077> ;
    dcat:landingPage "https://www.legislation.gov.au/F2021L00304/asmade/2021-03-24/text/original/epub/OEBPS/document_1/document_1.html#_Toc65844077"^^xsd:anyURI ;
    dcat:theme legcons:Division .

F2021L00304:73 a legcons:Division,
        owl:Class,
        dcat:Resource ;
    rdfs:label "Division - D73 Division 2 General"@en-AU ;
    dct:hasPart F2021L00304:74 ;
    dct:isPartOf F2021L00304:70 ;
    dct:isReferencedBy F2021L00304: ;
    rdfs:comment "Division 2 General - Abrievated Graph Key: D73"@en-AU ;
    skos:broader F2021L00304:74 ;
    skos:definition "Division 2 General"@en-AU ;
    skos:narrower F2021L00304:70 ;
    skos:prefLabel "Division D73"@en-AU ;
    dcat:accessURL <https://www.legislation.gov.au/F2021L00304/asmade/2021-03-24/text/original/epub/OEBPS/document_1/document_1.html#_Toc65844079> ;
    dcat:landingPage "https://www.legislation.gov.au/F2021L00304/asmade/2021-03-24/text/original/epub/OEBPS/document_1/document_1.html#_Toc65844079"^^xsd:anyURI ;
    dcat:theme legcons:Division .

F2021L00304:107 a legcons:Division,
        owl:Class,
        dcat:Resource ;
    rdfs:label "Division - D107 Division 8 Transfers"@en-AU ;
    dct:hasPart F2021L00304:108,
        F2021L00304:109 ;
    dct:isPartOf F2021L00304:70 ;
    dct:isReferencedBy F2021L00304: ;
    rdfs:comment "Division 8 Transfers - Abrievated Graph Key: D107"@en-AU ;
    skos:broader F2021L00304:108,
        F2021L00304:109 ;
    skos:definition "Division 8 Transfers"@en-AU ;
    skos:narrower F2021L00304:70 ;
    skos:prefLabel "Division D107"@en-AU ;
    dcat:accessURL <https://www.legislation.gov.au/F2021L00304/asmade/2021-03-24/text/original/epub/OEBPS/document_1/document_1.html#_Toc65844113> ;
    dcat:landingPage "https://www.legislation.gov.au/F2021L00304/asmade/2021-03-24/text/original/epub/OEBPS/document_1/document_1.html#_Toc65844113"^^xsd:anyURI ;
    dcat:theme legcons:Division .

F2021L00304:118 a legcons:Part,
        owl:Class,
        dcat:Resource ;
    rdfs:label "Part - P118 Part 4 Variation of approved arrangement"@en-AU ;
    dct:hasPart F2021L00304:119,
        F2021L00304:122 ;
    dct:isPartOf F2021L00304:63 ;
    dct:isReferencedBy F2021L00304: ;
    rdfs:comment "Part 4 Variation of approved arrangement - Abrievated Graph Key: P118"@en-AU ;
    skos:broader F2021L00304:119,
        F2021L00304:122 ;
    skos:definition "Part 4 Variation of approved arrangement"@en-AU ;
    skos:narrower F2021L00304:63 ;
    skos:prefLabel "Part P118"@en-AU ;
    dcat:accessURL <https://www.legislation.gov.au/F2021L00304/asmade/2021-03-24/text/original/epub/OEBPS/document_1/document_1.html#_Toc65844124> ;
    dcat:landingPage "https://www.legislation.gov.au/F2021L00304/asmade/2021-03-24/text/original/epub/OEBPS/document_1/document_1.html#_Toc65844124"^^xsd:anyURI ;
    dcat:theme legcons:Part .

F2021L00304:119 a legcons:Division,
        owl:Class,
        dcat:Resource ;
    rdfs:label "Division - D119 Division 1 Variations by holder"@en-AU ;
    dct:hasPart F2021L00304:120,
        F2021L00304:121 ;
    dct:isPartOf F2021L00304:118 ;
    dct:isReferencedBy F2021L00304: ;
    rdfs:comment "Division 1 Variations by holder - Abrievated Graph Key: D119"@en-AU ;
    skos:broader F2021L00304:120,
        F2021L00304:121 ;
    skos:definition "Division 1 Variations by holder"@en-AU ;
    skos:narrower F2021L00304:118 ;
    skos:prefLabel "Division D119"@en-AU ;
    dcat:accessURL <https://www.legislation.gov.au/F2021L00304/asmade/2021-03-24/text/original/epub/OEBPS/document_1/document_1.html#_Toc65844125> ;
    dcat:landingPage "https://www.legislation.gov.au/F2021L00304/asmade/2021-03-24/text/original/epub/OEBPS/document_1/document_1.html#_Toc65844125"^^xsd:anyURI ;
    dcat:theme legcons:Division .

F2021L00304:12 a legcons:Division,
        owl:Class,
        dcat:Resource ;
    rdfs:label "Division - D12 Division 1 Prescribed goods"@en-AU ;
    dct:hasPart F2021L00304:13,
        F2021L00304:14 ;
    dct:isPartOf F2021L00304:11 ;
    dct:isReferencedBy F2021L00304: ;
    rdfs:comment "Division 1 Prescribed goods - Abrievated Graph Key: D12"@en-AU ;
    skos:broader F2021L00304:13,
        F2021L00304:14 ;
    skos:definition "Division 1 Prescribed goods"@en-AU ;
    skos:narrower F2021L00304:11 ;
    skos:prefLabel "Division D12"@en-AU ;
    dcat:accessURL <https://www.legislation.gov.au/F2021L00304/asmade/2021-03-24/text/original/epub/OEBPS/document_1/document_1.html#_Toc65844018> ;
    dcat:landingPage "https://www.legislation.gov.au/F2021L00304/asmade/2021-03-24/text/original/epub/OEBPS/document_1/document_1.html#_Toc65844018"^^xsd:anyURI ;
    dcat:theme legcons:Division .

F2021L00304:129 a legcons:Part,
        owl:Class,
        dcat:Resource ;
    rdfs:label "Part - P129 Part 1 Issue of export permit"@en-AU ;
    dct:hasPart F2021L00304:130,
        F2021L00304:131 ;
    dct:isPartOf F2021L00304:128 ;
    dct:isReferencedBy F2021L00304: ;
    rdfs:comment "Part 1 Issue of export permit - Abrievated Graph Key: P129"@en-AU ;
    skos:broader F2021L00304:130,
        F2021L00304:131 ;
    skos:definition "Part 1 Issue of export permit"@en-AU ;
    skos:narrower F2021L00304:128 ;
    skos:prefLabel "Part P129"@en-AU ;
    dcat:accessURL <https://www.legislation.gov.au/F2021L00304/asmade/2021-03-24/text/original/epub/OEBPS/document_1/document_1.html#_Toc65844135> ;
    dcat:landingPage "https://www.legislation.gov.au/F2021L00304/asmade/2021-03-24/text/original/epub/OEBPS/document_1/document_1.html#_Toc65844135"^^xsd:anyURI ;
    dcat:theme legcons:Part .

F2021L00304:140 a legcons:Part,
        owl:Class,
        dcat:Resource ;
    rdfs:label "Part - P140 Part 4 Applications for export permits"@en-AU ;
    dct:hasPart F2021L00304:141,
        F2021L00304:142 ;
    dct:isPartOf F2021L00304:128 ;
    dct:isReferencedBy F2021L00304: ;
    rdfs:comment "Part 4 Applications for export permits - Abrievated Graph Key: P140"@en-AU ;
    skos:broader F2021L00304:141,
        F2021L00304:142 ;
    skos:definition "Part 4 Applications for export permits"@en-AU ;
    skos:narrower F2021L00304:128 ;
    skos:prefLabel "Part P140"@en-AU ;
    dcat:accessURL <https://www.legislation.gov.au/F2021L00304/asmade/2021-03-24/text/original/epub/OEBPS/document_1/document_1.html#_Toc65844146> ;
    dcat:landingPage "https://www.legislation.gov.au/F2021L00304/asmade/2021-03-24/text/original/epub/OEBPS/document_1/document_1.html#_Toc65844146"^^xsd:anyURI ;
    dcat:theme legcons:Part .

F2021L00304:185 a legcons:Division,
        owl:Class,
        dcat:Resource ;
    rdfs:label "Division - D185 Division 1 General"@en-AU ;
    dct:hasPart F2021L00304:186,
        F2021L00304:187 ;
    dct:isPartOf F2021L00304:184 ;
    dct:isReferencedBy F2021L00304: ;
    rdfs:comment "Division 1 General - Abrievated Graph Key: D185"@en-AU ;
    skos:broader F2021L00304:186,
        F2021L00304:187 ;
    skos:definition "Division 1 General"@en-AU ;
    skos:narrower F2021L00304:184 ;
    skos:prefLabel "Division D185"@en-AU ;
    dcat:accessURL <https://www.legislation.gov.au/F2021L00304/asmade/2021-03-24/text/original/epub/OEBPS/document_1/document_1.html#_Toc65844191> ;
    dcat:landingPage "https://www.legislation.gov.au/F2021L00304/asmade/2021-03-24/text/original/epub/OEBPS/document_1/document_1.html#_Toc65844191"^^xsd:anyURI ;
    dcat:theme legcons:Division .

F2021L00304:208 a legcons:Division,
        owl:Class,
        dcat:Resource ;
    rdfs:label "Division - D208 Division 2 Carrying out assessments etc"@en-AU ;
    dct:hasPart F2021L00304:209,
        F2021L00304:210 ;
    dct:isPartOf F2021L00304:205 ;
    dct:isReferencedBy F2021L00304: ;
    rdfs:comment "Division 2 Carrying out assessments etc - Abrievated Graph Key: D208"@en-AU ;
    skos:broader F2021L00304:209,
        F2021L00304:210 ;
    skos:definition "Division 2 Carrying out assessments etc"@en-AU ;
    skos:narrower F2021L00304:205 ;
    skos:prefLabel "Division D208"@en-AU ;
    dcat:accessURL <https://www.legislation.gov.au/F2021L00304/asmade/2021-03-24/text/original/epub/OEBPS/document_1/document_1.html#_Toc65844214> ;
    dcat:landingPage "https://www.legislation.gov.au/F2021L00304/asmade/2021-03-24/text/original/epub/OEBPS/document_1/document_1.html#_Toc65844214"^^xsd:anyURI ;
    dcat:theme legcons:Division .

F2021L00304:253 a legcons:Part,
        owl:Class,
        dcat:Resource ;
    rdfs:label "Part - P253 Part 3 Samples"@en-AU ;
    dct:hasPart F2021L00304:254,
        F2021L00304:255 ;
    dct:isPartOf F2021L00304:240 ;
    dct:isReferencedBy F2021L00304: ;
    rdfs:comment "Part 3 Samples - Abrievated Graph Key: P253"@en-AU ;
    skos:broader F2021L00304:254,
        F2021L00304:255 ;
    skos:definition "Part 3 Samples"@en-AU ;
    skos:narrower F2021L00304:240 ;
    skos:prefLabel "Part P253"@en-AU ;
    dcat:accessURL <https://www.legislation.gov.au/F2021L00304/asmade/2021-03-24/text/original/epub/OEBPS/document_1/document_1.html#_Toc65844259> ;
    dcat:landingPage "https://www.legislation.gov.au/F2021L00304/asmade/2021-03-24/text/original/epub/OEBPS/document_1/document_1.html#_Toc65844259"^^xsd:anyURI ;
    dcat:theme legcons:Part .

F2021L00304:256 a legcons:Part,
        owl:Class,
        dcat:Resource ;
    rdfs:label "Part - P256 Part 4 Damaged or destroyed milk or milk products"@en-AU ;
    dct:hasPart F2021L00304:257,
        F2021L00304:258 ;
    dct:isPartOf F2021L00304:240 ;
    dct:isReferencedBy F2021L00304: ;
    rdfs:comment "Part 4 Damaged or destroyed milk or milk products - Abrievated Graph Key: P256"@en-AU ;
    skos:broader F2021L00304:257,
        F2021L00304:258 ;
    skos:definition "Part 4 Damaged or destroyed milk or milk products"@en-AU ;
    skos:narrower F2021L00304:240 ;
    skos:prefLabel "Part P256"@en-AU ;
    dcat:accessURL <https://www.legislation.gov.au/F2021L00304/asmade/2021-03-24/text/original/epub/OEBPS/document_1/document_1.html#_Toc65844262> ;
    dcat:landingPage "https://www.legislation.gov.au/F2021L00304/asmade/2021-03-24/text/original/epub/OEBPS/document_1/document_1.html#_Toc65844262"^^xsd:anyURI ;
    dcat:theme legcons:Part .

F2021L00304:273 a legcons:Division,
        owl:Class,
        dcat:Resource ;
    rdfs:label "Division - D273 Division 3 Official marking devices"@en-AU ;
    dct:hasPart F2021L00304:274,
        F2021L00304:275 ;
    dct:isPartOf F2021L00304:266 ;
    dct:isReferencedBy F2021L00304: ;
    rdfs:comment "Division 3 Official marking devices - Abrievated Graph Key: D273"@en-AU ;
    skos:broader F2021L00304:274,
        F2021L00304:275 ;
    skos:definition "Division 3 Official marking devices"@en-AU ;
    skos:narrower F2021L00304:266 ;
    skos:prefLabel "Division D273"@en-AU ;
    dcat:accessURL <https://www.legislation.gov.au/F2021L00304/asmade/2021-03-24/text/original/epub/OEBPS/document_1/document_1.html#_Toc65844279> ;
    dcat:landingPage "https://www.legislation.gov.au/F2021L00304/asmade/2021-03-24/text/original/epub/OEBPS/document_1/document_1.html#_Toc65844279"^^xsd:anyURI ;
    dcat:theme legcons:Division .

F2021L00304:276 a legcons:Part,
        owl:Class,
        dcat:Resource ;
    rdfs:label "Part - P276 Part 4 Powers and officials"@en-AU ;
    dct:hasPart F2021L00304:277,
        F2021L00304:281 ;
    dct:isPartOf F2021L00304:261 ;
    dct:isReferencedBy F2021L00304: ;
    rdfs:comment "Part 4 Powers and officials - Abrievated Graph Key: P276"@en-AU ;
    skos:broader F2021L00304:277,
        F2021L00304:281 ;
    skos:definition "Part 4 Powers and officials"@en-AU ;
    skos:narrower F2021L00304:261 ;
    skos:prefLabel "Part P276"@en-AU ;
    dcat:accessURL <https://www.legislation.gov.au/F2021L00304/asmade/2021-03-24/text/original/epub/OEBPS/document_1/document_1.html#_Toc65844282> ;
    dcat:landingPage "https://www.legislation.gov.au/F2021L00304/asmade/2021-03-24/text/original/epub/OEBPS/document_1/document_1.html#_Toc65844282"^^xsd:anyURI ;
    dcat:theme legcons:Part .

F2021L00304:35 a legcons:Part,
        owl:Class,
        dcat:Resource ;
    rdfs:label "Part - P35 Part 1 Requirements for registration"@en-AU ;
    dct:hasPart F2021L00304:36,
        F2021L00304:46 ;
    dct:isPartOf F2021L00304:34 ;
    dct:isReferencedBy F2021L00304: ;
    rdfs:comment "Part 1 Requirements for registration - Abrievated Graph Key: P35"@en-AU ;
    skos:broader F2021L00304:36,
        F2021L00304:46 ;
    skos:definition "Part 1 Requirements for registration"@en-AU ;
    skos:narrower F2021L00304:34 ;
    skos:prefLabel "Part P35"@en-AU ;
    dcat:accessURL <https://www.legislation.gov.au/F2021L00304/asmade/2021-03-24/text/original/epub/OEBPS/document_1/document_1.html#_Toc65844041> ;
    dcat:landingPage "https://www.legislation.gov.au/F2021L00304/asmade/2021-03-24/text/original/epub/OEBPS/document_1/document_1.html#_Toc65844041"^^xsd:anyURI ;
    dcat:theme legcons:Part .

F2021L00304:46 a legcons:Division,
        owl:Class,
        dcat:Resource ;
    rdfs:label "Division - D46 Division 2 Other requirements"@en-AU ;
    dct:hasPart F2021L00304:47,
        F2021L00304:48 ;
    dct:isPartOf F2021L00304:35 ;
    dct:isReferencedBy F2021L00304: ;
    rdfs:comment "Division 2 Other requirements - Abrievated Graph Key: D46"@en-AU ;
    skos:broader F2021L00304:47,
        F2021L00304:48 ;
    skos:definition "Division 2 Other requirements"@en-AU ;
    skos:narrower F2021L00304:35 ;
    skos:prefLabel "Division D46"@en-AU ;
    dcat:accessURL <https://www.legislation.gov.au/F2021L00304/asmade/2021-03-24/text/original/epub/OEBPS/document_1/document_1.html#_Toc65844052> ;
    dcat:landingPage "https://www.legislation.gov.au/F2021L00304/asmade/2021-03-24/text/original/epub/OEBPS/document_1/document_1.html#_Toc65844052"^^xsd:anyURI ;
    dcat:theme legcons:Division .

F2021L00304:53 a legcons:Part,
        owl:Class,
        dcat:Resource ;
    rdfs:label "Part - P53 Part 3 Renewal of registration"@en-AU ;
    dct:hasPart F2021L00304:54,
        F2021L00304:55 ;
    dct:isPartOf F2021L00304:34 ;
    dct:isReferencedBy F2021L00304: ;
    rdfs:comment "Part 3 Renewal of registration - Abrievated Graph Key: P53"@en-AU ;
    skos:broader F2021L00304:54,
        F2021L00304:55 ;
    skos:definition "Part 3 Renewal of registration"@en-AU ;
    skos:narrower F2021L00304:34 ;
    skos:prefLabel "Part P53"@en-AU ;
    dcat:accessURL <https://www.legislation.gov.au/F2021L00304/asmade/2021-03-24/text/original/epub/OEBPS/document_1/document_1.html#_Toc65844059> ;
    dcat:landingPage "https://www.legislation.gov.au/F2021L00304/asmade/2021-03-24/text/original/epub/OEBPS/document_1/document_1.html#_Toc65844059"^^xsd:anyURI ;
    dcat:theme legcons:Part .

F2021L00304:56 a legcons:Part,
        owl:Class,
        dcat:Resource ;
    rdfs:label "Part - P56 Part 4 Suspension of registration"@en-AU ;
    dct:hasPart F2021L00304:57,
        F2021L00304:58 ;
    dct:isPartOf F2021L00304:34 ;
    dct:isReferencedBy F2021L00304: ;
    rdfs:comment "Part 4 Suspension of registration - Abrievated Graph Key: P56"@en-AU ;
    skos:broader F2021L00304:57,
        F2021L00304:58 ;
    skos:definition "Part 4 Suspension of registration"@en-AU ;
    skos:narrower F2021L00304:34 ;
    skos:prefLabel "Part P56"@en-AU ;
    dcat:accessURL <https://www.legislation.gov.au/F2021L00304/asmade/2021-03-24/text/original/epub/OEBPS/document_1/document_1.html#_Toc65844062> ;
    dcat:landingPage "https://www.legislation.gov.au/F2021L00304/asmade/2021-03-24/text/original/epub/OEBPS/document_1/document_1.html#_Toc65844062"^^xsd:anyURI ;
    dcat:theme legcons:Part .

F2021L00304:103 a legcons:Division,
        owl:Class,
        dcat:Resource ;
    rdfs:label "Division - D103 Division 7 Segregation identification security traceability and integrity"@en-AU ;
    dct:hasPart F2021L00304:104,
        F2021L00304:105,
        F2021L00304:106 ;
    dct:isPartOf F2021L00304:70 ;
    dct:isReferencedBy F2021L00304: ;
    rdfs:comment "Division 7 Segregation identification security traceability and integrity - Abrievated Graph Key: D103"@en-AU ;
    skos:broader F2021L00304:104,
        F2021L00304:105,
        F2021L00304:106 ;
    skos:definition "Division 7 Segregation identification security traceability and integrity"@en-AU ;
    skos:narrower F2021L00304:70 ;
    skos:prefLabel "Division D103"@en-AU ;
    dcat:accessURL <https://www.legislation.gov.au/F2021L00304/asmade/2021-03-24/text/original/epub/OEBPS/document_1/document_1.html#_Toc65844109> ;
    dcat:landingPage "https://www.legislation.gov.au/F2021L00304/asmade/2021-03-24/text/original/epub/OEBPS/document_1/document_1.html#_Toc65844109"^^xsd:anyURI ;
    dcat:theme legcons:Division .

F2021L00304:124 a legcons:Part,
        owl:Class,
        dcat:Resource ;
    rdfs:label "Part - P124 Part 5 Matters relating to applications"@en-AU ;
    dct:hasPart F2021L00304:125,
        F2021L00304:126,
        F2021L00304:127 ;
    dct:isPartOf F2021L00304:63 ;
    dct:isReferencedBy F2021L00304: ;
    rdfs:comment "Part 5 Matters relating to applications - Abrievated Graph Key: P124"@en-AU ;
    skos:broader F2021L00304:125,
        F2021L00304:126,
        F2021L00304:127 ;
    skos:definition "Part 5 Matters relating to applications"@en-AU ;
    skos:narrower F2021L00304:63 ;
    skos:prefLabel "Part P124"@en-AU ;
    dcat:accessURL <https://www.legislation.gov.au/F2021L00304/asmade/2021-03-24/text/original/epub/OEBPS/document_1/document_1.html#_Toc65844130> ;
    dcat:landingPage "https://www.legislation.gov.au/F2021L00304/asmade/2021-03-24/text/original/epub/OEBPS/document_1/document_1.html#_Toc65844130"^^xsd:anyURI ;
    dcat:theme legcons:Part .

F2021L00304:128 a legcons:Chapter,
        owl:Class,
        dcat:Resource ;
    rdfs:label "Chapter - C128 Chapter 7 Export permits"@en-AU ;
    dct:hasPart F2021L00304:129,
        F2021L00304:132,
        F2021L00304:136,
        F2021L00304:140 ;
    dct:isReferencedBy F2021L00304: ;
    rdfs:comment "Chapter 7 Export permits - Abrievated Graph Key: C128"@en-AU ;
    skos:broader F2021L00304:129,
        F2021L00304:132,
        F2021L00304:136,
        F2021L00304:140 ;
    skos:definition "Chapter 7 Export permits"@en-AU ;
    skos:prefLabel "Chapter C128"@en-AU ;
    dcat:accessURL <https://www.legislation.gov.au/F2021L00304/asmade/2021-03-24/text/original/epub/OEBPS/document_1/document_1.html#_Toc65844134> ;
    dcat:landingPage "https://www.legislation.gov.au/F2021L00304/asmade/2021-03-24/text/original/epub/OEBPS/document_1/document_1.html#_Toc65844134"^^xsd:anyURI ;
    dcat:theme legcons:Chapter .

F2021L00304:132 a legcons:Part,
        owl:Class,
        dcat:Resource ;
    rdfs:label "Part - P132 Part 2 Variation suspension and revocation of export permit"@en-AU ;
    dct:hasPart F2021L00304:133,
        F2021L00304:134,
        F2021L00304:135 ;
    dct:isPartOf F2021L00304:128 ;
    dct:isReferencedBy F2021L00304: ;
    rdfs:comment "Part 2 Variation suspension and revocation of export permit - Abrievated Graph Key: P132"@en-AU ;
    skos:broader F2021L00304:133,
        F2021L00304:134,
        F2021L00304:135 ;
    skos:definition "Part 2 Variation suspension and revocation of export permit"@en-AU ;
    skos:narrower F2021L00304:128 ;
    skos:prefLabel "Part P132"@en-AU ;
    dcat:accessURL <https://www.legislation.gov.au/F2021L00304/asmade/2021-03-24/text/original/epub/OEBPS/document_1/document_1.html#_Toc65844138> ;
    dcat:landingPage "https://www.legislation.gov.au/F2021L00304/asmade/2021-03-24/text/original/epub/OEBPS/document_1/document_1.html#_Toc65844138"^^xsd:anyURI ;
    dcat:theme legcons:Part .

F2021L00304:136 a legcons:Part,
        owl:Class,
        dcat:Resource ;
    rdfs:label "Part - P136 Part 3 Other matters"@en-AU ;
    dct:hasPart F2021L00304:137,
        F2021L00304:138,
        F2021L00304:139 ;
    dct:isPartOf F2021L00304:128 ;
    dct:isReferencedBy F2021L00304: ;
    rdfs:comment "Part 3 Other matters - Abrievated Graph Key: P136"@en-AU ;
    skos:broader F2021L00304:137,
        F2021L00304:138,
        F2021L00304:139 ;
    skos:definition "Part 3 Other matters"@en-AU ;
    skos:narrower F2021L00304:128 ;
    skos:prefLabel "Part P136"@en-AU ;
    dcat:accessURL <https://www.legislation.gov.au/F2021L00304/asmade/2021-03-24/text/original/epub/OEBPS/document_1/document_1.html#_Toc65844142> ;
    dcat:landingPage "https://www.legislation.gov.au/F2021L00304/asmade/2021-03-24/text/original/epub/OEBPS/document_1/document_1.html#_Toc65844142"^^xsd:anyURI ;
    dcat:theme legcons:Part .

F2021L00304:144 a legcons:Part,
        owl:Class,
        dcat:Resource ;
    rdfs:label "Part - P144 Part 1 Trade descriptions"@en-AU ;
    dct:hasPart F2021L00304:145,
        F2021L00304:146,
        F2021L00304:147 ;
    dct:isPartOf F2021L00304:143 ;
    dct:isReferencedBy F2021L00304: ;
    rdfs:comment "Part 1 Trade descriptions - Abrievated Graph Key: P144"@en-AU ;
    skos:broader F2021L00304:145,
        F2021L00304:146,
        F2021L00304:147 ;
    skos:definition "Part 1 Trade descriptions"@en-AU ;
    skos:narrower F2021L00304:143 ;
    skos:prefLabel "Part P144"@en-AU ;
    dcat:accessURL <https://www.legislation.gov.au/F2021L00304/asmade/2021-03-24/text/original/epub/OEBPS/document_1/document_1.html#_Toc65844150> ;
    dcat:landingPage "https://www.legislation.gov.au/F2021L00304/asmade/2021-03-24/text/original/epub/OEBPS/document_1/document_1.html#_Toc65844150"^^xsd:anyURI ;
    dcat:theme legcons:Part .

F2021L00304:172 a legcons:Division,
        owl:Class,
        dcat:Resource ;
    rdfs:label "Division - D172 Division 3 Marks resembling official marks"@en-AU ;
    dct:hasPart F2021L00304:173,
        F2021L00304:174,
        F2021L00304:175 ;
    dct:isPartOf F2021L00304:148 ;
    dct:isReferencedBy F2021L00304: ;
    rdfs:comment "Division 3 Marks resembling official marks - Abrievated Graph Key: D172"@en-AU ;
    skos:broader F2021L00304:173,
        F2021L00304:174,
        F2021L00304:175 ;
    skos:definition "Division 3 Marks resembling official marks"@en-AU ;
    skos:narrower F2021L00304:148 ;
    skos:prefLabel "Division D172"@en-AU ;
    dcat:accessURL <https://www.legislation.gov.au/F2021L00304/asmade/2021-03-24/text/original/epub/OEBPS/document_1/document_1.html#_Toc65844178> ;
    dcat:landingPage "https://www.legislation.gov.au/F2021L00304/asmade/2021-03-24/text/original/epub/OEBPS/document_1/document_1.html#_Toc65844178"^^xsd:anyURI ;
    dcat:theme legcons:Division .

F2021L00304:183 a legcons:Chapter,
        owl:Class,
        dcat:Resource ;
    rdfs:label "Chapter - C183 Chapter 9 Powers and officials"@en-AU ;
    dct:hasPart F2021L00304:184,
        F2021L00304:205,
        F2021L00304:223,
        F2021L00304:225 ;
    dct:isReferencedBy F2021L00304: ;
    rdfs:comment "Chapter 9 Powers and officials - Abrievated Graph Key: C183"@en-AU ;
    skos:broader F2021L00304:184,
        F2021L00304:205,
        F2021L00304:223,
        F2021L00304:225 ;
    skos:definition "Chapter 9 Powers and officials"@en-AU ;
    skos:prefLabel "Chapter C183"@en-AU ;
    dcat:accessURL <https://www.legislation.gov.au/F2021L00304/asmade/2021-03-24/text/original/epub/OEBPS/document_1/document_1.html#_Toc65844189> ;
    dcat:landingPage "https://www.legislation.gov.au/F2021L00304/asmade/2021-03-24/text/original/epub/OEBPS/document_1/document_1.html#_Toc65844189"^^xsd:anyURI ;
    dcat:theme legcons:Chapter .

F2021L00304:184 a legcons:Part,
        owl:Class,
        dcat:Resource ;
    rdfs:label "Part - P184 Part 1 Audits"@en-AU ;
    dct:hasPart F2021L00304:185,
        F2021L00304:188,
        F2021L00304:193 ;
    dct:isPartOf F2021L00304:183 ;
    dct:isReferencedBy F2021L00304: ;
    rdfs:comment "Part 1 Audits - Abrievated Graph Key: P184"@en-AU ;
    skos:broader F2021L00304:185,
        F2021L00304:188,
        F2021L00304:193 ;
    skos:definition "Part 1 Audits"@en-AU ;
    skos:narrower F2021L00304:183 ;
    skos:prefLabel "Part P184"@en-AU ;
    dcat:accessURL <https://www.legislation.gov.au/F2021L00304/asmade/2021-03-24/text/original/epub/OEBPS/document_1/document_1.html#_Toc65844190> ;
    dcat:landingPage "https://www.legislation.gov.au/F2021L00304/asmade/2021-03-24/text/original/epub/OEBPS/document_1/document_1.html#_Toc65844190"^^xsd:anyURI ;
    dcat:theme legcons:Part .

F2021L00304:205 a legcons:Part,
        owl:Class,
        dcat:Resource ;
    rdfs:label "Part - P205 Part 2 Assessments"@en-AU ;
    dct:hasPart F2021L00304:206,
        F2021L00304:208,
        F2021L00304:211 ;
    dct:isPartOf F2021L00304:183 ;
    dct:isReferencedBy F2021L00304: ;
    rdfs:comment "Part 2 Assessments - Abrievated Graph Key: P205"@en-AU ;
    skos:broader F2021L00304:206,
        F2021L00304:208,
        F2021L00304:211 ;
    skos:definition "Part 2 Assessments"@en-AU ;
    skos:narrower F2021L00304:183 ;
    skos:prefLabel "Part P205"@en-AU ;
    dcat:accessURL <https://www.legislation.gov.au/F2021L00304/asmade/2021-03-24/text/original/epub/OEBPS/document_1/document_1.html#_Toc65844211> ;
    dcat:landingPage "https://www.legislation.gov.au/F2021L00304/asmade/2021-03-24/text/original/epub/OEBPS/document_1/document_1.html#_Toc65844211"^^xsd:anyURI ;
    dcat:theme legcons:Part .

F2021L00304:261 a legcons:Chapter,
        owl:Class,
        dcat:Resource ;
    rdfs:label "Chapter - C261 Chapter 12 Transitional provisions"@en-AU ;
    dct:hasPart F2021L00304:262,
        F2021L00304:264,
        F2021L00304:266,
        F2021L00304:276 ;
    dct:isReferencedBy F2021L00304: ;
    rdfs:comment "Chapter 12 Transitional provisions - Abrievated Graph Key: C261"@en-AU ;
    skos:broader F2021L00304:262,
        F2021L00304:264,
        F2021L00304:266,
        F2021L00304:276 ;
    skos:definition "Chapter 12 Transitional provisions"@en-AU ;
    skos:prefLabel "Chapter C261"@en-AU ;
    dcat:accessURL <https://www.legislation.gov.au/F2021L00304/asmade/2021-03-24/text/original/epub/OEBPS/document_1/document_1.html#_Toc65844267> ;
    dcat:landingPage "https://www.legislation.gov.au/F2021L00304/asmade/2021-03-24/text/original/epub/OEBPS/document_1/document_1.html#_Toc65844267"^^xsd:anyURI ;
    dcat:theme legcons:Chapter .

F2021L00304:266 a legcons:Part,
        owl:Class,
        dcat:Resource ;
    rdfs:label "Part - P266 Part 3 Other matters relating to export"@en-AU ;
    dct:hasPart F2021L00304:267,
        F2021L00304:269,
        F2021L00304:273 ;
    dct:isPartOf F2021L00304:261 ;
    dct:isReferencedBy F2021L00304: ;
    rdfs:comment "Part 3 Other matters relating to export - Abrievated Graph Key: P266"@en-AU ;
    skos:broader F2021L00304:267,
        F2021L00304:269,
        F2021L00304:273 ;
    skos:definition "Part 3 Other matters relating to export"@en-AU ;
    skos:narrower F2021L00304:261 ;
    skos:prefLabel "Part P266"@en-AU ;
    dcat:accessURL <https://www.legislation.gov.au/F2021L00304/asmade/2021-03-24/text/original/epub/OEBPS/document_1/document_1.html#_Toc65844272> ;
    dcat:landingPage "https://www.legislation.gov.au/F2021L00304/asmade/2021-03-24/text/original/epub/OEBPS/document_1/document_1.html#_Toc65844272"^^xsd:anyURI ;
    dcat:theme legcons:Part .

F2021L00304:269 a legcons:Division,
        owl:Class,
        dcat:Resource ;
    rdfs:label "Division - D269 Division 2 Official marks"@en-AU ;
    dct:hasPart F2021L00304:270,
        F2021L00304:271,
        F2021L00304:272 ;
    dct:isPartOf F2021L00304:266 ;
    dct:isReferencedBy F2021L00304: ;
    rdfs:comment "Division 2 Official marks - Abrievated Graph Key: D269"@en-AU ;
    skos:broader F2021L00304:270,
        F2021L00304:271,
        F2021L00304:272 ;
    skos:definition "Division 2 Official marks"@en-AU ;
    skos:narrower F2021L00304:266 ;
    skos:prefLabel "Division D269"@en-AU ;
    dcat:accessURL <https://www.legislation.gov.au/F2021L00304/asmade/2021-03-24/text/original/epub/OEBPS/document_1/document_1.html#_Toc65844275> ;
    dcat:landingPage "https://www.legislation.gov.au/F2021L00304/asmade/2021-03-24/text/original/epub/OEBPS/document_1/document_1.html#_Toc65844275"^^xsd:anyURI ;
    dcat:theme legcons:Division .

F2021L00304:277 a legcons:Division,
        owl:Class,
        dcat:Resource ;
    rdfs:label "Division - D277 Division 1 Approved auditors"@en-AU ;
    dct:hasPart F2021L00304:278,
        F2021L00304:279,
        F2021L00304:280 ;
    dct:isPartOf F2021L00304:276 ;
    dct:isReferencedBy F2021L00304: ;
    rdfs:comment "Division 1 Approved auditors - Abrievated Graph Key: D277"@en-AU ;
    skos:broader F2021L00304:278,
        F2021L00304:279,
        F2021L00304:280 ;
    skos:definition "Division 1 Approved auditors"@en-AU ;
    skos:narrower F2021L00304:276 ;
    skos:prefLabel "Division D277"@en-AU ;
    dcat:accessURL <https://www.legislation.gov.au/F2021L00304/asmade/2021-03-24/text/original/epub/OEBPS/document_1/document_1.html#_Toc65844283> ;
    dcat:landingPage "https://www.legislation.gov.au/F2021L00304/asmade/2021-03-24/text/original/epub/OEBPS/document_1/document_1.html#_Toc65844283"^^xsd:anyURI ;
    dcat:theme legcons:Division .

F2021L00304:49 a legcons:Part,
        owl:Class,
        dcat:Resource ;
    rdfs:label "Part - P49 Part 2 Conditions of registration"@en-AU ;
    dct:hasPart F2021L00304:50,
        F2021L00304:51,
        F2021L00304:52 ;
    dct:isPartOf F2021L00304:34 ;
    dct:isReferencedBy F2021L00304: ;
    rdfs:comment "Part 2 Conditions of registration - Abrievated Graph Key: P49"@en-AU ;
    skos:broader F2021L00304:50,
        F2021L00304:51,
        F2021L00304:52 ;
    skos:definition "Part 2 Conditions of registration"@en-AU ;
    skos:narrower F2021L00304:34 ;
    skos:prefLabel "Part P49"@en-AU ;
    dcat:accessURL <https://www.legislation.gov.au/F2021L00304/asmade/2021-03-24/text/original/epub/OEBPS/document_1/document_1.html#_Toc65844055> ;
    dcat:landingPage "https://www.legislation.gov.au/F2021L00304/asmade/2021-03-24/text/original/epub/OEBPS/document_1/document_1.html#_Toc65844055"^^xsd:anyURI ;
    dcat:theme legcons:Part .

F2021L00304:59 a legcons:Part,
        owl:Class,
        dcat:Resource ;
    rdfs:label "Part - P59 Part 5 Matters relating to applications"@en-AU ;
    dct:hasPart F2021L00304:60,
        F2021L00304:61,
        F2021L00304:62 ;
    dct:isPartOf F2021L00304:34 ;
    dct:isReferencedBy F2021L00304: ;
    rdfs:comment "Part 5 Matters relating to applications - Abrievated Graph Key: P59"@en-AU ;
    skos:broader F2021L00304:60,
        F2021L00304:61,
        F2021L00304:62 ;
    skos:definition "Part 5 Matters relating to applications"@en-AU ;
    skos:narrower F2021L00304:34 ;
    skos:prefLabel "Part P59"@en-AU ;
    dcat:accessURL <https://www.legislation.gov.au/F2021L00304/asmade/2021-03-24/text/original/epub/OEBPS/document_1/document_1.html#_Toc65844065> ;
    dcat:landingPage "https://www.legislation.gov.au/F2021L00304/asmade/2021-03-24/text/original/epub/OEBPS/document_1/document_1.html#_Toc65844065"^^xsd:anyURI ;
    dcat:theme legcons:Part .

F2021L00304:11 a legcons:Part,
        owl:Class,
        dcat:Resource ;
    rdfs:label "Part - P11 Part 1 Goods"@en-AU ;
    dct:hasPart F2021L00304:12,
        F2021L00304:15,
        F2021L00304:16,
        F2021L00304:17 ;
    dct:isPartOf F2021L00304:10 ;
    dct:isReferencedBy F2021L00304: ;
    rdfs:comment "Part 1 Goods - Abrievated Graph Key: P11"@en-AU ;
    skos:broader F2021L00304:12,
        F2021L00304:15,
        F2021L00304:16,
        F2021L00304:17 ;
    skos:definition "Part 1 Goods"@en-AU ;
    skos:narrower F2021L00304:10 ;
    skos:prefLabel "Part P11"@en-AU ;
    dcat:accessURL <https://www.legislation.gov.au/F2021L00304/asmade/2021-03-24/text/original/epub/OEBPS/document_1/document_1.html#_Toc65844017> ;
    dcat:landingPage "https://www.legislation.gov.au/F2021L00304/asmade/2021-03-24/text/original/epub/OEBPS/document_1/document_1.html#_Toc65844017"^^xsd:anyURI ;
    dcat:theme legcons:Part .

F2021L00304:148 a legcons:Part,
        owl:Class,
        dcat:Resource ;
    rdfs:label "Part - P148 Part 2 Official marks"@en-AU ;
    dct:hasPart F2021L00304:149,
        F2021L00304:159,
        F2021L00304:172,
        F2021L00304:176 ;
    dct:isPartOf F2021L00304:143 ;
    dct:isReferencedBy F2021L00304: ;
    rdfs:comment "Part 2 Official marks - Abrievated Graph Key: P148"@en-AU ;
    skos:broader F2021L00304:149,
        F2021L00304:159,
        F2021L00304:172,
        F2021L00304:176 ;
    skos:definition "Part 2 Official marks"@en-AU ;
    skos:narrower F2021L00304:143 ;
    skos:prefLabel "Part P148"@en-AU ;
    dcat:accessURL <https://www.legislation.gov.au/F2021L00304/asmade/2021-03-24/text/original/epub/OEBPS/document_1/document_1.html#_Toc65844154> ;
    dcat:landingPage "https://www.legislation.gov.au/F2021L00304/asmade/2021-03-24/text/original/epub/OEBPS/document_1/document_1.html#_Toc65844154"^^xsd:anyURI ;
    dcat:theme legcons:Part .

F2021L00304:188 a legcons:Division,
        owl:Class,
        dcat:Resource ;
    rdfs:label "Division - D188 Division 2 Conduct of audit etc"@en-AU ;
    dct:hasPart F2021L00304:189,
        F2021L00304:190,
        F2021L00304:191,
        F2021L00304:192 ;
    dct:isPartOf F2021L00304:184 ;
    dct:isReferencedBy F2021L00304: ;
    rdfs:comment "Division 2 Conduct of audit etc - Abrievated Graph Key: D188"@en-AU ;
    skos:broader F2021L00304:189,
        F2021L00304:190,
        F2021L00304:191,
        F2021L00304:192 ;
    skos:definition "Division 2 Conduct of audit etc"@en-AU ;
    skos:narrower F2021L00304:184 ;
    skos:prefLabel "Division D188"@en-AU ;
    dcat:accessURL <https://www.legislation.gov.au/F2021L00304/asmade/2021-03-24/text/original/epub/OEBPS/document_1/document_1.html#_Toc65844194> ;
    dcat:landingPage "https://www.legislation.gov.au/F2021L00304/asmade/2021-03-24/text/original/epub/OEBPS/document_1/document_1.html#_Toc65844194"^^xsd:anyURI ;
    dcat:theme legcons:Division .

F2021L00304:225 a legcons:Part,
        owl:Class,
        dcat:Resource ;
    rdfs:label "Part - P225 Part 4 Authorised officers"@en-AU ;
    dct:hasPart F2021L00304:226,
        F2021L00304:228,
        F2021L00304:233,
        F2021L00304:235 ;
    dct:isPartOf F2021L00304:183 ;
    dct:isReferencedBy F2021L00304: ;
    rdfs:comment "Part 4 Authorised officers - Abrievated Graph Key: P225"@en-AU ;
    skos:broader F2021L00304:226,
        F2021L00304:228,
        F2021L00304:233,
        F2021L00304:235 ;
    skos:definition "Part 4 Authorised officers"@en-AU ;
    skos:narrower F2021L00304:183 ;
    skos:prefLabel "Part P225"@en-AU ;
    dcat:accessURL <https://www.legislation.gov.au/F2021L00304/asmade/2021-03-24/text/original/epub/OEBPS/document_1/document_1.html#_Toc65844231> ;
    dcat:landingPage "https://www.legislation.gov.au/F2021L00304/asmade/2021-03-24/text/original/epub/OEBPS/document_1/document_1.html#_Toc65844231"^^xsd:anyURI ;
    dcat:theme legcons:Part .

F2021L00304:228 a legcons:Division,
        owl:Class,
        dcat:Resource ;
    rdfs:label "Division - D228 Division 2 Functions and powers"@en-AU ;
    dct:hasPart F2021L00304:229,
        F2021L00304:230,
        F2021L00304:231,
        F2021L00304:232 ;
    dct:isPartOf F2021L00304:225 ;
    dct:isReferencedBy F2021L00304: ;
    rdfs:comment "Division 2 Functions and powers - Abrievated Graph Key: D228"@en-AU ;
    skos:broader F2021L00304:229,
        F2021L00304:230,
        F2021L00304:231,
        F2021L00304:232 ;
    skos:definition "Division 2 Functions and powers"@en-AU ;
    skos:narrower F2021L00304:225 ;
    skos:prefLabel "Division D228"@en-AU ;
    dcat:accessURL <https://www.legislation.gov.au/F2021L00304/asmade/2021-03-24/text/original/epub/OEBPS/document_1/document_1.html#_Toc65844234> ;
    dcat:landingPage "https://www.legislation.gov.au/F2021L00304/asmade/2021-03-24/text/original/epub/OEBPS/document_1/document_1.html#_Toc65844234"^^xsd:anyURI ;
    dcat:theme legcons:Division .

F2021L00304:240 a legcons:Chapter,
        owl:Class,
        dcat:Resource ;
    rdfs:label "Chapter - C240 Chapter 11 Miscellaneous"@en-AU ;
    dct:hasPart F2021L00304:241,
        F2021L00304:243,
        F2021L00304:253,
        F2021L00304:256,
        F2021L00304:259 ;
    dct:isReferencedBy F2021L00304: ;
    rdfs:comment "Chapter 11 Miscellaneous - Abrievated Graph Key: C240"@en-AU ;
    skos:broader F2021L00304:241,
        F2021L00304:243,
        F2021L00304:253,
        F2021L00304:256,
        F2021L00304:259 ;
    skos:definition "Chapter 11 Miscellaneous"@en-AU ;
    skos:prefLabel "Chapter C240"@en-AU ;
    dcat:accessURL <https://www.legislation.gov.au/F2021L00304/asmade/2021-03-24/text/original/epub/OEBPS/document_1/document_1.html#_Toc65844246> ;
    dcat:landingPage "https://www.legislation.gov.au/F2021L00304/asmade/2021-03-24/text/original/epub/OEBPS/document_1/document_1.html#_Toc65844246"^^xsd:anyURI ;
    dcat:theme legcons:Chapter .

F2021L00304:34 a legcons:Chapter,
        owl:Class,
        dcat:Resource ;
    rdfs:label "Chapter - C34 Chapter 4 Registered establishments"@en-AU ;
    dct:hasPart F2021L00304:35,
        F2021L00304:49,
        F2021L00304:53,
        F2021L00304:56,
        F2021L00304:59 ;
    dct:isReferencedBy F2021L00304: ;
    rdfs:comment "Chapter 4 Registered establishments - Abrievated Graph Key: C34"@en-AU ;
    skos:broader F2021L00304:35,
        F2021L00304:49,
        F2021L00304:53,
        F2021L00304:56,
        F2021L00304:59 ;
    skos:definition "Chapter 4 Registered establishments"@en-AU ;
    skos:prefLabel "Chapter C34"@en-AU ;
    dcat:accessURL <https://www.legislation.gov.au/F2021L00304/asmade/2021-03-24/text/original/epub/OEBPS/document_1/document_1.html#_Toc65844040> ;
    dcat:landingPage "https://www.legislation.gov.au/F2021L00304/asmade/2021-03-24/text/original/epub/OEBPS/document_1/document_1.html#_Toc65844040"^^xsd:anyURI ;
    dcat:theme legcons:Chapter .

F2021L00304:63 a legcons:Chapter,
        owl:Class,
        dcat:Resource ;
    rdfs:label "Chapter - C63 Chapter 5 Approved arrangements"@en-AU ;
    dct:hasPart F2021L00304:116,
        F2021L00304:118,
        F2021L00304:124,
        F2021L00304:64,
        F2021L00304:70 ;
    dct:isReferencedBy F2021L00304: ;
    rdfs:comment "Chapter 5 Approved arrangements - Abrievated Graph Key: C63"@en-AU ;
    skos:broader F2021L00304:116,
        F2021L00304:118,
        F2021L00304:124,
        F2021L00304:64,
        F2021L00304:70 ;
    skos:definition "Chapter 5 Approved arrangements"@en-AU ;
    skos:prefLabel "Chapter C63"@en-AU ;
    dcat:accessURL <https://www.legislation.gov.au/F2021L00304/asmade/2021-03-24/text/original/epub/OEBPS/document_1/document_1.html#_Toc65844069> ;
    dcat:landingPage "https://www.legislation.gov.au/F2021L00304/asmade/2021-03-24/text/original/epub/OEBPS/document_1/document_1.html#_Toc65844069"^^xsd:anyURI ;
    dcat:theme legcons:Chapter .

F2021L00304:96 a legcons:Division,
        owl:Class,
        dcat:Resource ;
    rdfs:label "Division - D96 Division 5 Trade descriptions"@en-AU ;
    dct:hasPart F2021L00304:100,
        F2021L00304:97,
        F2021L00304:98,
        F2021L00304:99 ;
    dct:isPartOf F2021L00304:70 ;
    dct:isReferencedBy F2021L00304: ;
    rdfs:comment "Division 5 Trade descriptions - Abrievated Graph Key: D96"@en-AU ;
    skos:broader F2021L00304:100,
        F2021L00304:97,
        F2021L00304:98,
        F2021L00304:99 ;
    skos:definition "Division 5 Trade descriptions"@en-AU ;
    skos:narrower F2021L00304:70 ;
    skos:prefLabel "Division D96"@en-AU ;
    dcat:accessURL <https://www.legislation.gov.au/F2021L00304/asmade/2021-03-24/text/original/epub/OEBPS/document_1/document_1.html#_Toc65844102> ;
    dcat:landingPage "https://www.legislation.gov.au/F2021L00304/asmade/2021-03-24/text/original/epub/OEBPS/document_1/document_1.html#_Toc65844102"^^xsd:anyURI ;
    dcat:theme legcons:Division .

F2021L00304:110 a legcons:Division,
        owl:Class,
        dcat:Resource ;
    rdfs:label "Division - D110 Division 9 Management practicesexport operations"@en-AU ;
    dct:hasPart F2021L00304:111,
        F2021L00304:112,
        F2021L00304:113,
        F2021L00304:114,
        F2021L00304:115 ;
    dct:isPartOf F2021L00304:70 ;
    dct:isReferencedBy F2021L00304: ;
    rdfs:comment "Division 9 Management practicesexport operations - Abrievated Graph Key: D110"@en-AU ;
    skos:broader F2021L00304:111,
        F2021L00304:112,
        F2021L00304:113,
        F2021L00304:114,
        F2021L00304:115 ;
    skos:definition "Division 9 Management practicesexport operations"@en-AU ;
    skos:narrower F2021L00304:70 ;
    skos:prefLabel "Division D110"@en-AU ;
    dcat:accessURL <https://www.legislation.gov.au/F2021L00304/asmade/2021-03-24/text/original/epub/OEBPS/document_1/document_1.html#_Toc65844116> ;
    dcat:landingPage "https://www.legislation.gov.au/F2021L00304/asmade/2021-03-24/text/original/epub/OEBPS/document_1/document_1.html#_Toc65844116"^^xsd:anyURI ;
    dcat:theme legcons:Division .

F2021L00304:64 a legcons:Part,
        owl:Class,
        dcat:Resource ;
    rdfs:label "Part - P64 Part 1 Requirements for approval"@en-AU ;
    dct:hasPart F2021L00304:65,
        F2021L00304:66,
        F2021L00304:67,
        F2021L00304:68,
        F2021L00304:69 ;
    dct:isPartOf F2021L00304:63 ;
    dct:isReferencedBy F2021L00304: ;
    rdfs:comment "Part 1 Requirements for approval - Abrievated Graph Key: P64"@en-AU ;
    skos:broader F2021L00304:65,
        F2021L00304:66,
        F2021L00304:67,
        F2021L00304:68,
        F2021L00304:69 ;
    skos:definition "Part 1 Requirements for approval"@en-AU ;
    skos:narrower F2021L00304:63 ;
    skos:prefLabel "Part P64"@en-AU ;
    dcat:accessURL <https://www.legislation.gov.au/F2021L00304/asmade/2021-03-24/text/original/epub/OEBPS/document_1/document_1.html#_Toc65844070> ;
    dcat:landingPage "https://www.legislation.gov.au/F2021L00304/asmade/2021-03-24/text/original/epub/OEBPS/document_1/document_1.html#_Toc65844070"^^xsd:anyURI ;
    dcat:theme legcons:Part .

F2021L00304:75 a legcons:Division,
        owl:Class,
        dcat:Resource ;
    rdfs:label "Division - D75 Division 3 Operational hygiene"@en-AU ;
    dct:hasPart F2021L00304:76,
        F2021L00304:77,
        F2021L00304:78,
        F2021L00304:79,
        F2021L00304:80 ;
    dct:isPartOf F2021L00304:70 ;
    dct:isReferencedBy F2021L00304: ;
    rdfs:comment "Division 3 Operational hygiene - Abrievated Graph Key: D75"@en-AU ;
    skos:broader F2021L00304:76,
        F2021L00304:77,
        F2021L00304:78,
        F2021L00304:79,
        F2021L00304:80 ;
    skos:definition "Division 3 Operational hygiene"@en-AU ;
    skos:narrower F2021L00304:70 ;
    skos:prefLabel "Division D75"@en-AU ;
    dcat:accessURL <https://www.legislation.gov.au/F2021L00304/asmade/2021-03-24/text/original/epub/OEBPS/document_1/document_1.html#_Toc65844081> ;
    dcat:landingPage "https://www.legislation.gov.au/F2021L00304/asmade/2021-03-24/text/original/epub/OEBPS/document_1/document_1.html#_Toc65844081"^^xsd:anyURI ;
    dcat:theme legcons:Division .

F2021L00304:176 a legcons:Division,
        owl:Class,
        dcat:Resource ;
    rdfs:label "Division - D176 Division 4 Official marking devices"@en-AU ;
    dct:hasPart F2021L00304:177,
        F2021L00304:178,
        F2021L00304:179,
        F2021L00304:180,
        F2021L00304:181,
        F2021L00304:182 ;
    dct:isPartOf F2021L00304:148 ;
    dct:isReferencedBy F2021L00304: ;
    rdfs:comment "Division 4 Official marking devices - Abrievated Graph Key: D176"@en-AU ;
    skos:broader F2021L00304:177,
        F2021L00304:178,
        F2021L00304:179,
        F2021L00304:180,
        F2021L00304:181,
        F2021L00304:182 ;
    skos:definition "Division 4 Official marking devices"@en-AU ;
    skos:narrower F2021L00304:148 ;
    skos:prefLabel "Division D176"@en-AU ;
    dcat:accessURL <https://www.legislation.gov.au/F2021L00304/asmade/2021-03-24/text/original/epub/OEBPS/document_1/document_1.html#_Toc65844182> ;
    dcat:landingPage "https://www.legislation.gov.au/F2021L00304/asmade/2021-03-24/text/original/epub/OEBPS/document_1/document_1.html#_Toc65844182"^^xsd:anyURI ;
    dcat:theme legcons:Division .

F2021L00304:1 a legcons:Chapter,
        owl:Class,
        dcat:Resource ;
    rdfs:label "Chapter - C1 Chapter 1 Preliminary"@en-AU ;
    dct:hasPart F2021L00304:2,
        F2021L00304:3,
        F2021L00304:4,
        F2021L00304:5,
        F2021L00304:6,
        F2021L00304:7,
        F2021L00304:8,
        F2021L00304:9 ;
    dct:isReferencedBy F2021L00304: ;
    rdfs:comment "Chapter 1 Preliminary - Abrievated Graph Key: C1"@en-AU ;
    skos:broader F2021L00304:2,
        F2021L00304:3,
        F2021L00304:4,
        F2021L00304:5,
        F2021L00304:6,
        F2021L00304:7,
        F2021L00304:8,
        F2021L00304:9 ;
    skos:definition "Chapter 1 Preliminary"@en-AU ;
    skos:prefLabel "Chapter C1"@en-AU ;
    dcat:accessURL <https://www.legislation.gov.au/F2021L00304/asmade/2021-03-24/text/original/epub/OEBPS/document_1/document_1.html#_Toc65844007> ;
    dcat:landingPage "https://www.legislation.gov.au/F2021L00304/asmade/2021-03-24/text/original/epub/OEBPS/document_1/document_1.html#_Toc65844007"^^xsd:anyURI ;
    dcat:theme legcons:Chapter .

F2021L00304:149 a legcons:Division,
        owl:Class,
        dcat:Resource ;
    rdfs:label "Division - D149 Division 1 Marks that are official marks"@en-AU ;
    dct:hasPart F2021L00304:150,
        F2021L00304:151,
        F2021L00304:152,
        F2021L00304:153,
        F2021L00304:154,
        F2021L00304:155,
        F2021L00304:156,
        F2021L00304:157,
        F2021L00304:158 ;
    dct:isPartOf F2021L00304:148 ;
    dct:isReferencedBy F2021L00304: ;
    rdfs:comment "Division 1 Marks that are official marks - Abrievated Graph Key: D149"@en-AU ;
    skos:broader F2021L00304:150,
        F2021L00304:151,
        F2021L00304:152,
        F2021L00304:153,
        F2021L00304:154,
        F2021L00304:155,
        F2021L00304:156,
        F2021L00304:157,
        F2021L00304:158 ;
    skos:definition "Division 1 Marks that are official marks"@en-AU ;
    skos:narrower F2021L00304:148 ;
    skos:prefLabel "Division D149"@en-AU ;
    dcat:accessURL <https://www.legislation.gov.au/F2021L00304/asmade/2021-03-24/text/original/epub/OEBPS/document_1/document_1.html#_Toc65844155> ;
    dcat:landingPage "https://www.legislation.gov.au/F2021L00304/asmade/2021-03-24/text/original/epub/OEBPS/document_1/document_1.html#_Toc65844155"^^xsd:anyURI ;
    dcat:theme legcons:Division .

F2021L00304:243 a legcons:Part,
        owl:Class,
        dcat:Resource ;
    rdfs:label "Part - P243 Part 2 Records"@en-AU ;
    dct:hasPart F2021L00304:244,
        F2021L00304:245,
        F2021L00304:246,
        F2021L00304:247,
        F2021L00304:248,
        F2021L00304:249,
        F2021L00304:250,
        F2021L00304:251,
        F2021L00304:252 ;
    dct:isPartOf F2021L00304:240 ;
    dct:isReferencedBy F2021L00304: ;
    rdfs:comment "Part 2 Records - Abrievated Graph Key: P243"@en-AU ;
    skos:broader F2021L00304:244,
        F2021L00304:245,
        F2021L00304:246,
        F2021L00304:247,
        F2021L00304:248,
        F2021L00304:249,
        F2021L00304:250,
        F2021L00304:251,
        F2021L00304:252 ;
    skos:definition "Part 2 Records"@en-AU ;
    skos:narrower F2021L00304:240 ;
    skos:prefLabel "Part P243"@en-AU ;
    dcat:accessURL <https://www.legislation.gov.au/F2021L00304/asmade/2021-03-24/text/original/epub/OEBPS/document_1/document_1.html#_Toc65844249> ;
    dcat:landingPage "https://www.legislation.gov.au/F2021L00304/asmade/2021-03-24/text/original/epub/OEBPS/document_1/document_1.html#_Toc65844249"^^xsd:anyURI ;
    dcat:theme legcons:Part .

F2021L00304:36 a legcons:Division,
        owl:Class,
        dcat:Resource ;
    rdfs:label "Division - D36 Division 1 Requirements relating to construction equipment and facilities"@en-AU ;
    dct:hasPart F2021L00304:37,
        F2021L00304:38,
        F2021L00304:39,
        F2021L00304:40,
        F2021L00304:41,
        F2021L00304:42,
        F2021L00304:43,
        F2021L00304:44,
        F2021L00304:45 ;
    dct:isPartOf F2021L00304:35 ;
    dct:isReferencedBy F2021L00304: ;
    rdfs:comment "Division 1 Requirements relating to construction equipment and facilities - Abrievated Graph Key: D36"@en-AU ;
    skos:broader F2021L00304:37,
        F2021L00304:38,
        F2021L00304:39,
        F2021L00304:40,
        F2021L00304:41,
        F2021L00304:42,
        F2021L00304:43,
        F2021L00304:44,
        F2021L00304:45 ;
    skos:definition "Division 1 Requirements relating to construction equipment and facilities"@en-AU ;
    skos:narrower F2021L00304:35 ;
    skos:prefLabel "Division D36"@en-AU ;
    dcat:accessURL <https://www.legislation.gov.au/F2021L00304/asmade/2021-03-24/text/original/epub/OEBPS/document_1/document_1.html#_Toc65844042> ;
    dcat:landingPage "https://www.legislation.gov.au/F2021L00304/asmade/2021-03-24/text/original/epub/OEBPS/document_1/document_1.html#_Toc65844042"^^xsd:anyURI ;
    dcat:theme legcons:Division .

F2021L00304:70 a legcons:Part,
        owl:Class,
        dcat:Resource ;
    rdfs:label "Part - P70 Part 2 Conditions of approved arrangement"@en-AU ;
    dct:hasPart F2021L00304:101,
        F2021L00304:103,
        F2021L00304:107,
        F2021L00304:110,
        F2021L00304:71,
        F2021L00304:73,
        F2021L00304:75,
        F2021L00304:81,
        F2021L00304:96 ;
    dct:isPartOf F2021L00304:63 ;
    dct:isReferencedBy F2021L00304: ;
    rdfs:comment "Part 2 Conditions of approved arrangement - Abrievated Graph Key: P70"@en-AU ;
    skos:broader F2021L00304:101,
        F2021L00304:103,
        F2021L00304:107,
        F2021L00304:110,
        F2021L00304:71,
        F2021L00304:73,
        F2021L00304:75,
        F2021L00304:81,
        F2021L00304:96 ;
    skos:definition "Part 2 Conditions of approved arrangement"@en-AU ;
    skos:narrower F2021L00304:63 ;
    skos:prefLabel "Part P70"@en-AU ;
    dcat:accessURL <https://www.legislation.gov.au/F2021L00304/asmade/2021-03-24/text/original/epub/OEBPS/document_1/document_1.html#_Toc65844076> ;
    dcat:landingPage "https://www.legislation.gov.au/F2021L00304/asmade/2021-03-24/text/original/epub/OEBPS/document_1/document_1.html#_Toc65844076"^^xsd:anyURI ;
    dcat:theme legcons:Part .

F2021L00304:193 a legcons:Division,
        owl:Class,
        dcat:Resource ;
    rdfs:label "Division - D193 Division 3 Approved auditors"@en-AU ;
    dct:hasPart F2021L00304:194,
        F2021L00304:195,
        F2021L00304:196,
        F2021L00304:197,
        F2021L00304:198,
        F2021L00304:199,
        F2021L00304:200,
        F2021L00304:201,
        F2021L00304:202,
        F2021L00304:203,
        F2021L00304:204 ;
    dct:isPartOf F2021L00304:184 ;
    dct:isReferencedBy F2021L00304: ;
    rdfs:comment "Division 3 Approved auditors - Abrievated Graph Key: D193"@en-AU ;
    skos:broader F2021L00304:194,
        F2021L00304:195,
        F2021L00304:196,
        F2021L00304:197,
        F2021L00304:198,
        F2021L00304:199,
        F2021L00304:200,
        F2021L00304:201,
        F2021L00304:202,
        F2021L00304:203,
        F2021L00304:204 ;
    skos:definition "Division 3 Approved auditors"@en-AU ;
    skos:narrower F2021L00304:184 ;
    skos:prefLabel "Division D193"@en-AU ;
    dcat:accessURL <https://www.legislation.gov.au/F2021L00304/asmade/2021-03-24/text/original/epub/OEBPS/document_1/document_1.html#_Toc65844199> ;
    dcat:landingPage "https://www.legislation.gov.au/F2021L00304/asmade/2021-03-24/text/original/epub/OEBPS/document_1/document_1.html#_Toc65844199"^^xsd:anyURI ;
    dcat:theme legcons:Division .

F2021L00304:211 a legcons:Division,
        owl:Class,
        dcat:Resource ;
    rdfs:label "Division - D211 Division 3 Approved assessors"@en-AU ;
    dct:hasPart F2021L00304:212,
        F2021L00304:213,
        F2021L00304:214,
        F2021L00304:215,
        F2021L00304:216,
        F2021L00304:217,
        F2021L00304:218,
        F2021L00304:219,
        F2021L00304:220,
        F2021L00304:221,
        F2021L00304:222 ;
    dct:isPartOf F2021L00304:205 ;
    dct:isReferencedBy F2021L00304: ;
    rdfs:comment "Division 3 Approved assessors - Abrievated Graph Key: D211"@en-AU ;
    skos:broader F2021L00304:212,
        F2021L00304:213,
        F2021L00304:214,
        F2021L00304:215,
        F2021L00304:216,
        F2021L00304:217,
        F2021L00304:218,
        F2021L00304:219,
        F2021L00304:220,
        F2021L00304:221,
        F2021L00304:222 ;
    skos:definition "Division 3 Approved assessors"@en-AU ;
    skos:narrower F2021L00304:205 ;
    skos:prefLabel "Division D211"@en-AU ;
    dcat:accessURL <https://www.legislation.gov.au/F2021L00304/asmade/2021-03-24/text/original/epub/OEBPS/document_1/document_1.html#_Toc65844217> ;
    dcat:landingPage "https://www.legislation.gov.au/F2021L00304/asmade/2021-03-24/text/original/epub/OEBPS/document_1/document_1.html#_Toc65844217"^^xsd:anyURI ;
    dcat:theme legcons:Division .

F2021L00304:159 a legcons:Division,
        owl:Class,
        dcat:Resource ;
    rdfs:label "Division - D159 Division 2 General rules relating to official marks"@en-AU ;
    dct:hasPart F2021L00304:160,
        F2021L00304:161,
        F2021L00304:162,
        F2021L00304:163,
        F2021L00304:164,
        F2021L00304:165,
        F2021L00304:166,
        F2021L00304:167,
        F2021L00304:168,
        F2021L00304:169,
        F2021L00304:170,
        F2021L00304:171 ;
    dct:isPartOf F2021L00304:148 ;
    dct:isReferencedBy F2021L00304: ;
    rdfs:comment "Division 2 General rules relating to official marks - Abrievated Graph Key: D159"@en-AU ;
    skos:broader F2021L00304:160,
        F2021L00304:161,
        F2021L00304:162,
        F2021L00304:163,
        F2021L00304:164,
        F2021L00304:165,
        F2021L00304:166,
        F2021L00304:167,
        F2021L00304:168,
        F2021L00304:169,
        F2021L00304:170,
        F2021L00304:171 ;
    skos:definition "Division 2 General rules relating to official marks"@en-AU ;
    skos:narrower F2021L00304:148 ;
    skos:prefLabel "Division D159"@en-AU ;
    dcat:accessURL <https://www.legislation.gov.au/F2021L00304/asmade/2021-03-24/text/original/epub/OEBPS/document_1/document_1.html#_Toc65844165> ;
    dcat:landingPage "https://www.legislation.gov.au/F2021L00304/asmade/2021-03-24/text/original/epub/OEBPS/document_1/document_1.html#_Toc65844165"^^xsd:anyURI ;
    dcat:theme legcons:Division .

F2021L00304:81 a legcons:Division,
        owl:Class,
        dcat:Resource ;
    rdfs:label "Division - D81 Division 4 Preparation and transport"@en-AU ;
    dct:hasPart F2021L00304:82,
        F2021L00304:83,
        F2021L00304:84,
        F2021L00304:85,
        F2021L00304:86,
        F2021L00304:87,
        F2021L00304:88,
        F2021L00304:89,
        F2021L00304:90,
        F2021L00304:91,
        F2021L00304:92,
        F2021L00304:93,
        F2021L00304:94,
        F2021L00304:95 ;
    dct:isPartOf F2021L00304:70 ;
    dct:isReferencedBy F2021L00304: ;
    rdfs:comment "Division 4 Preparation and transport - Abrievated Graph Key: D81"@en-AU ;
    skos:broader F2021L00304:82,
        F2021L00304:83,
        F2021L00304:84,
        F2021L00304:85,
        F2021L00304:86,
        F2021L00304:87,
        F2021L00304:88,
        F2021L00304:89,
        F2021L00304:90,
        F2021L00304:91,
        F2021L00304:92,
        F2021L00304:93,
        F2021L00304:94,
        F2021L00304:95 ;
    skos:definition "Division 4 Preparation and transport"@en-AU ;
    skos:narrower F2021L00304:70 ;
    skos:prefLabel "Division D81"@en-AU ;
    dcat:accessURL <https://www.legislation.gov.au/F2021L00304/asmade/2021-03-24/text/original/epub/OEBPS/document_1/document_1.html#_Toc65844087> ;
    dcat:landingPage "https://www.legislation.gov.au/F2021L00304/asmade/2021-03-24/text/original/epub/OEBPS/document_1/document_1.html#_Toc65844087"^^xsd:anyURI ;
    dcat:theme legcons:Division .

F2021L00304:10 a legcons:Chapter,
        owl:Class,
        dcat:Resource ;
    rdfs:label "Chapter - C10 Chapter 2 Exporting goods"@en-AU ;
    dct:hasPart F2021L00304:11,
        F2021L00304:18,
        F2021L00304:19,
        F2021L00304:20,
        F2021L00304:21,
        F2021L00304:22,
        F2021L00304:23,
        F2021L00304:24,
        F2021L00304:25,
        F2021L00304:26,
        F2021L00304:27,
        F2021L00304:28,
        F2021L00304:29,
        F2021L00304:30,
        F2021L00304:31,
        F2021L00304:32,
        F2021L00304:33 ;
    dct:isReferencedBy F2021L00304: ;
    rdfs:comment "Chapter 2 Exporting goods - Abrievated Graph Key: C10"@en-AU ;
    skos:broader F2021L00304:11,
        F2021L00304:18,
        F2021L00304:19,
        F2021L00304:20,
        F2021L00304:21,
        F2021L00304:22,
        F2021L00304:23,
        F2021L00304:24,
        F2021L00304:25,
        F2021L00304:26,
        F2021L00304:27,
        F2021L00304:28,
        F2021L00304:29,
        F2021L00304:30,
        F2021L00304:31,
        F2021L00304:32,
        F2021L00304:33 ;
    skos:definition "Chapter 2 Exporting goods"@en-AU ;
    skos:prefLabel "Chapter C10"@en-AU ;
    dcat:accessURL <https://www.legislation.gov.au/F2021L00304/asmade/2021-03-24/text/original/epub/OEBPS/document_1/document_1.html#_Toc65844016> ;
    dcat:landingPage "https://www.legislation.gov.au/F2021L00304/asmade/2021-03-24/text/original/epub/OEBPS/document_1/document_1.html#_Toc65844016"^^xsd:anyURI ;
    dcat:theme legcons:Chapter .

F2021L00304: a owl:Class,
        dcat:Dataset,
        dcat:Resource ;
    rdfs:label "Export Control (Milk and Milk Products) Rules 2021" ;
    dct:Jurisdiction " Department of Agriculture, Fisheries and Forestry "@en-AU ;
    dct:created "2024-08-30T15:13:47.828539"^^xsd:dateTime ;
    dct:creator "https://orcid.org/0009-0007-8434-7325"^^xsd:anyURI ;
    dct:date "2021-03-24T00:00:00+11:00"^^xsd:dateTime ;
    dct:description "Export Control (Milk and Milk Products) Rules 2021"@en-AU ;
    dct:identifier "https://www.legislation.gov.au/F2021L00304/asmade"^^xsd:anyURI ;
    dct:license <https://creativecommons.org/licenses/by-sa/4.0/> ;
    dct:source "scheme=AGLSTERMS.AglsAgent; corporateName=Office Parliamentary Counsel; address=Locked Bag 30 Kingston ACT 2604; contact=+61 2 6120 1400"@en-AU ;
    dct:subject "Export Control (Milk and Milk Products) Rules 2021"@en-AU ;
    dct:title "Export Control (Milk and Milk Products) Rules 2021"@en-AU ;
    owl:imports legcons: ;
    dcat:theme legcons:Chapter,
        legcons:Division,
        legcons:Item,
        legcons:Part ;
    schema:identifier "F2021L00304" ;
    schema:status "In force" ;
    schema:version "F2021L00304" .

