@prefix F2021L00339: <http://example.org/au/leg/dataset/F2021L00339/> .
@prefix dcat: <http://www.w3.org/ns/dcat#> .
@prefix dct: <http://purl.org/dc/terms/> .
@prefix legcons: <http://example.org/au/leg/concepts/> .
@prefix owl: <http://www.w3.org/2002/07/owl#> .
@prefix rdfs: <http://www.w3.org/2000/01/rdf-schema#> .
@prefix schema: <https://schema.org/> .
@prefix skos: <http://www.w3.org/2004/02/skos/core#> .
@prefix xsd: <http://www.w3.org/2001/XMLSchema#> .

F2021L00339:100 a legcons:Item,
        owl:Class,
        dcat:Resource ;
    rdfs:label "Item - I100 11 11  Circumstances in which relevant Commonwealth liability of a person is taken to have been paid"@en-AU ;
    dct:isPartOf F2021L00339:99 ;
    dct:isReferencedBy F2021L00339: ;
    rdfs:comment "11 11  Circumstances in which relevant Commonwealth liability of a person is taken to have been paid - Abrievated Graph Key: I100"@en-AU ;
    skos:definition "11 11  Circumstances in which relevant Commonwealth liability of a person is taken to have been paid"@en-AU ;
    skos:narrower F2021L00339:99 ;
    skos:prefLabel "Item I100"@en-AU ;
    dcat:accessURL <https://www.legislation.gov.au/F2021L00339/2023-08-04/2023-08-04/text/original/epub/OEBPS/document_1/document_1.html#_Toc143615237> ;
    dcat:landingPage "https://www.legislation.gov.au/F2021L00339/2023-08-04/2023-08-04/text/original/epub/OEBPS/document_1/document_1.html#_Toc143615237"^^xsd:anyURI ;
    dcat:theme legcons:Item .

F2021L00339:103 a legcons:Item,
        owl:Class,
        dcat:Resource ;
    rdfs:label "Item - I103 12 1  Definitions"@en-AU ;
    dct:isPartOf F2021L00339:102 ;
    dct:isReferencedBy F2021L00339: ;
    rdfs:comment "12 1  Definitions - Abrievated Graph Key: I103"@en-AU ;
    skos:definition "12 1  Definitions"@en-AU ;
    skos:narrower F2021L00339:102 ;
    skos:prefLabel "Item I103"@en-AU ;
    dcat:accessURL <https://www.legislation.gov.au/F2021L00339/2023-08-04/2023-08-04/text/original/epub/OEBPS/document_1/document_1.html#_Toc143615240> ;
    dcat:landingPage "https://www.legislation.gov.au/F2021L00339/2023-08-04/2023-08-04/text/original/epub/OEBPS/document_1/document_1.html#_Toc143615240"^^xsd:anyURI ;
    dcat:theme legcons:Item .

F2021L00339:105 a legcons:Item,
        owl:Class,
        dcat:Resource ;
    rdfs:label "Item - I105 12 2  QM certificate in force immediately before commencement time"@en-AU ;
    dct:isPartOf F2021L00339:104 ;
    dct:isReferencedBy F2021L00339: ;
    rdfs:comment "12 2  QM certificate in force immediately before commencement time - Abrievated Graph Key: I105"@en-AU ;
    skos:definition "12 2  QM certificate in force immediately before commencement time"@en-AU ;
    skos:narrower F2021L00339:104 ;
    skos:prefLabel "Item I105"@en-AU ;
    dcat:accessURL <https://www.legislation.gov.au/F2021L00339/2023-08-04/2023-08-04/text/original/epub/OEBPS/document_1/document_1.html#_Toc143615242> ;
    dcat:landingPage "https://www.legislation.gov.au/F2021L00339/2023-08-04/2023-08-04/text/original/epub/OEBPS/document_1/document_1.html#_Toc143615242"^^xsd:anyURI ;
    dcat:theme legcons:Item .

F2021L00339:106 a legcons:Item,
        owl:Class,
        dcat:Resource ;
    rdfs:label "Item - I106 12 3  Secretary may direct holder to vary continuing approved arrangement"@en-AU ;
    dct:isPartOf F2021L00339:104 ;
    dct:isReferencedBy F2021L00339: ;
    rdfs:comment "12 3  Secretary may direct holder to vary continuing approved arrangement - Abrievated Graph Key: I106"@en-AU ;
    skos:definition "12 3  Secretary may direct holder to vary continuing approved arrangement"@en-AU ;
    skos:narrower F2021L00339:104 ;
    skos:prefLabel "Item I106"@en-AU ;
    dcat:accessURL <https://www.legislation.gov.au/F2021L00339/2023-08-04/2023-08-04/text/original/epub/OEBPS/document_1/document_1.html#_Toc143615243> ;
    dcat:landingPage "https://www.legislation.gov.au/F2021L00339/2023-08-04/2023-08-04/text/original/epub/OEBPS/document_1/document_1.html#_Toc143615243"^^xsd:anyURI ;
    dcat:theme legcons:Item .

F2021L00339:107 a legcons:Item,
        owl:Class,
        dcat:Resource ;
    rdfs:label "Item - I107 12 4  Application for QM certificate made but not decided before commencement time"@en-AU ;
    dct:isPartOf F2021L00339:104 ;
    dct:isReferencedBy F2021L00339: ;
    rdfs:comment "12 4  Application for QM certificate made but not decided before commencement time - Abrievated Graph Key: I107"@en-AU ;
    skos:definition "12 4  Application for QM certificate made but not decided before commencement time"@en-AU ;
    skos:narrower F2021L00339:104 ;
    skos:prefLabel "Item I107"@en-AU ;
    dcat:accessURL <https://www.legislation.gov.au/F2021L00339/2023-08-04/2023-08-04/text/original/epub/OEBPS/document_1/document_1.html#_Toc143615244> ;
    dcat:landingPage "https://www.legislation.gov.au/F2021L00339/2023-08-04/2023-08-04/text/original/epub/OEBPS/document_1/document_1.html#_Toc143615244"^^xsd:anyURI ;
    dcat:theme legcons:Item .

F2021L00339:108 a legcons:Item,
        owl:Class,
        dcat:Resource ;
    rdfs:label "Item - I108 12 5  Application for approval of modification of QM system made but not decided before commencement time"@en-AU ;
    dct:isPartOf F2021L00339:104 ;
    dct:isReferencedBy F2021L00339: ;
    rdfs:comment "12 5  Application for approval of modification of QM system made but not decided before commencement time - Abrievated Graph Key: I108"@en-AU ;
    skos:definition "12 5  Application for approval of modification of QM system made but not decided before commencement time"@en-AU ;
    skos:narrower F2021L00339:104 ;
    skos:prefLabel "Item I108"@en-AU ;
    dcat:accessURL <https://www.legislation.gov.au/F2021L00339/2023-08-04/2023-08-04/text/original/epub/OEBPS/document_1/document_1.html#_Toc143615245> ;
    dcat:landingPage "https://www.legislation.gov.au/F2021L00339/2023-08-04/2023-08-04/text/original/epub/OEBPS/document_1/document_1.html#_Toc143615245"^^xsd:anyURI ;
    dcat:theme legcons:Item .

F2021L00339:109 a legcons:Item,
        owl:Class,
        dcat:Resource ;
    rdfs:label "Item - I109 12 6  Corrective action request given before commencement time"@en-AU ;
    dct:isPartOf F2021L00339:104 ;
    dct:isReferencedBy F2021L00339: ;
    rdfs:comment "12 6  Corrective action request given before commencement time - Abrievated Graph Key: I109"@en-AU ;
    skos:definition "12 6  Corrective action request given before commencement time"@en-AU ;
    skos:narrower F2021L00339:104 ;
    skos:prefLabel "Item I109"@en-AU ;
    dcat:accessURL <https://www.legislation.gov.au/F2021L00339/2023-08-04/2023-08-04/text/original/epub/OEBPS/document_1/document_1.html#_Toc143615246> ;
    dcat:landingPage "https://www.legislation.gov.au/F2021L00339/2023-08-04/2023-08-04/text/original/epub/OEBPS/document_1/document_1.html#_Toc143615246"^^xsd:anyURI ;
    dcat:theme legcons:Item .

F2021L00339:110 a legcons:Item,
        owl:Class,
        dcat:Resource ;
    rdfs:label "Item - I110 12 7  Modifications of the Act relating to applications"@en-AU ;
    dct:isPartOf F2021L00339:104 ;
    dct:isReferencedBy F2021L00339: ;
    rdfs:comment "12 7  Modifications of the Act relating to applications - Abrievated Graph Key: I110"@en-AU ;
    skos:definition "12 7  Modifications of the Act relating to applications"@en-AU ;
    skos:narrower F2021L00339:104 ;
    skos:prefLabel "Item I110"@en-AU ;
    dcat:accessURL <https://www.legislation.gov.au/F2021L00339/2023-08-04/2023-08-04/text/original/epub/OEBPS/document_1/document_1.html#_Toc143615247> ;
    dcat:landingPage "https://www.legislation.gov.au/F2021L00339/2023-08-04/2023-08-04/text/original/epub/OEBPS/document_1/document_1.html#_Toc143615247"^^xsd:anyURI ;
    dcat:theme legcons:Item .

F2021L00339:112 a legcons:Item,
        owl:Class,
        dcat:Resource ;
    rdfs:label "Item - I112 Endnote 1 About the endnotes"@en-AU ;
    dct:isPartOf F2021L00339:111 ;
    dct:isReferencedBy F2021L00339: ;
    rdfs:comment "Endnote 1 About the endnotes - Abrievated Graph Key: I112"@en-AU ;
    skos:definition "Endnote 1 About the endnotes"@en-AU ;
    skos:narrower F2021L00339:111 ;
    skos:prefLabel "Item I112"@en-AU ;
    dcat:accessURL <https://www.legislation.gov.au/F2021L00339/2023-08-04/2023-08-04/text/original/epub/OEBPS/document_1/document_1.html#_Toc143615249> ;
    dcat:landingPage "https://www.legislation.gov.au/F2021L00339/2023-08-04/2023-08-04/text/original/epub/OEBPS/document_1/document_1.html#_Toc143615249"^^xsd:anyURI ;
    dcat:theme legcons:Item .

F2021L00339:113 a legcons:Item,
        owl:Class,
        dcat:Resource ;
    rdfs:label "Item - I113 Endnote 2 Abbreviation key"@en-AU ;
    dct:isPartOf F2021L00339:111 ;
    dct:isReferencedBy F2021L00339: ;
    rdfs:comment "Endnote 2 Abbreviation key - Abrievated Graph Key: I113"@en-AU ;
    skos:definition "Endnote 2 Abbreviation key"@en-AU ;
    skos:narrower F2021L00339:111 ;
    skos:prefLabel "Item I113"@en-AU ;
    dcat:accessURL <https://www.legislation.gov.au/F2021L00339/2023-08-04/2023-08-04/text/original/epub/OEBPS/document_1/document_1.html#_Toc143615250> ;
    dcat:landingPage "https://www.legislation.gov.au/F2021L00339/2023-08-04/2023-08-04/text/original/epub/OEBPS/document_1/document_1.html#_Toc143615250"^^xsd:anyURI ;
    dcat:theme legcons:Item .

F2021L00339:114 a legcons:Item,
        owl:Class,
        dcat:Resource ;
    rdfs:label "Item - I114 Endnote 3 Legislation history"@en-AU ;
    dct:isPartOf F2021L00339:111 ;
    dct:isReferencedBy F2021L00339: ;
    rdfs:comment "Endnote 3 Legislation history - Abrievated Graph Key: I114"@en-AU ;
    skos:definition "Endnote 3 Legislation history"@en-AU ;
    skos:narrower F2021L00339:111 ;
    skos:prefLabel "Item I114"@en-AU ;
    dcat:accessURL <https://www.legislation.gov.au/F2021L00339/2023-08-04/2023-08-04/text/original/epub/OEBPS/document_1/document_1.html#_Toc143615251> ;
    dcat:landingPage "https://www.legislation.gov.au/F2021L00339/2023-08-04/2023-08-04/text/original/epub/OEBPS/document_1/document_1.html#_Toc143615251"^^xsd:anyURI ;
    dcat:theme legcons:Item .

F2021L00339:115 a legcons:Item,
        owl:Class,
        dcat:Resource ;
    rdfs:label "Item - I115 Endnote 4 Amendment history"@en-AU ;
    dct:isPartOf F2021L00339:111 ;
    dct:isReferencedBy F2021L00339: ;
    rdfs:comment "Endnote 4 Amendment history - Abrievated Graph Key: I115"@en-AU ;
    skos:definition "Endnote 4 Amendment history"@en-AU ;
    skos:narrower F2021L00339:111 ;
    skos:prefLabel "Item I115"@en-AU ;
    dcat:accessURL <https://www.legislation.gov.au/F2021L00339/2023-08-04/2023-08-04/text/original/epub/OEBPS/document_1/document_1.html#_Toc143615252> ;
    dcat:landingPage "https://www.legislation.gov.au/F2021L00339/2023-08-04/2023-08-04/text/original/epub/OEBPS/document_1/document_1.html#_Toc143615252"^^xsd:anyURI ;
    dcat:theme legcons:Item .

F2021L00339:12 a legcons:Item,
        owl:Class,
        dcat:Resource ;
    rdfs:label "Item - I12 2 1  Organic goods that are prescribed goods"@en-AU ;
    dct:isPartOf F2021L00339:11 ;
    dct:isReferencedBy F2021L00339: ;
    rdfs:comment "2 1  Organic goods that are prescribed goods - Abrievated Graph Key: I12"@en-AU ;
    skos:definition "2 1  Organic goods that are prescribed goods"@en-AU ;
    skos:narrower F2021L00339:11 ;
    skos:prefLabel "Item I12"@en-AU ;
    dcat:accessURL <https://www.legislation.gov.au/F2021L00339/2023-08-04/2023-08-04/text/original/epub/OEBPS/document_1/document_1.html#_Toc143615149> ;
    dcat:landingPage "https://www.legislation.gov.au/F2021L00339/2023-08-04/2023-08-04/text/original/epub/OEBPS/document_1/document_1.html#_Toc143615149"^^xsd:anyURI ;
    dcat:theme legcons:Item .

F2021L00339:13 a legcons:Item,
        owl:Class,
        dcat:Resource ;
    rdfs:label "Item - I13 2 2  Organic goods that are taken not to be prescribed goods"@en-AU ;
    dct:isPartOf F2021L00339:11 ;
    dct:isReferencedBy F2021L00339: ;
    rdfs:comment "2 2  Organic goods that are taken not to be prescribed goods - Abrievated Graph Key: I13"@en-AU ;
    skos:definition "2 2  Organic goods that are taken not to be prescribed goods"@en-AU ;
    skos:narrower F2021L00339:11 ;
    skos:prefLabel "Item I13"@en-AU ;
    dcat:accessURL <https://www.legislation.gov.au/F2021L00339/2023-08-04/2023-08-04/text/original/epub/OEBPS/document_1/document_1.html#_Toc143615150> ;
    dcat:landingPage "https://www.legislation.gov.au/F2021L00339/2023-08-04/2023-08-04/text/original/epub/OEBPS/document_1/document_1.html#_Toc143615150"^^xsd:anyURI ;
    dcat:theme legcons:Item .

F2021L00339:14 a legcons:Division,
        owl:Class,
        dcat:Resource ;
    rdfs:label "Division - D14 Division 2 Prohibited export and prescribed export conditions"@en-AU ;
    dct:isPartOf F2021L00339:10 ;
    dct:isReferencedBy F2021L00339: ;
    rdfs:comment "Division 2 Prohibited export and prescribed export conditions - Abrievated Graph Key: D14"@en-AU ;
    skos:definition "Division 2 Prohibited export and prescribed export conditions"@en-AU ;
    skos:narrower F2021L00339:10 ;
    skos:prefLabel "Division D14"@en-AU ;
    dcat:accessURL <https://www.legislation.gov.au/F2021L00339/2023-08-04/2023-08-04/text/original/epub/OEBPS/document_1/document_1.html#_Toc143615151> ;
    dcat:landingPage "https://www.legislation.gov.au/F2021L00339/2023-08-04/2023-08-04/text/original/epub/OEBPS/document_1/document_1.html#_Toc143615151"^^xsd:anyURI ;
    dcat:theme legcons:Division .

F2021L00339:15 a legcons:Item,
        owl:Class,
        dcat:Resource ;
    rdfs:label "Item - I15 2 3  Purpose and application of this Division"@en-AU ;
    dct:isPartOf F2021L00339:10 ;
    dct:isReferencedBy F2021L00339: ;
    rdfs:comment "2 3  Purpose and application of this Division - Abrievated Graph Key: I15"@en-AU ;
    skos:definition "2 3  Purpose and application of this Division"@en-AU ;
    skos:narrower F2021L00339:10 ;
    skos:prefLabel "Item I15"@en-AU ;
    dcat:accessURL <https://www.legislation.gov.au/F2021L00339/2023-08-04/2023-08-04/text/original/epub/OEBPS/document_1/document_1.html#_Toc143615152> ;
    dcat:landingPage "https://www.legislation.gov.au/F2021L00339/2023-08-04/2023-08-04/text/original/epub/OEBPS/document_1/document_1.html#_Toc143615152"^^xsd:anyURI ;
    dcat:theme legcons:Item .

F2021L00339:16 a legcons:Item,
        owl:Class,
        dcat:Resource ;
    rdfs:label "Item - I16 2 4  Export of prescribed organic goods is prohibited unless prescribed conditions are complied with"@en-AU ;
    dct:isPartOf F2021L00339:10 ;
    dct:isReferencedBy F2021L00339: ;
    rdfs:comment "2 4  Export of prescribed organic goods is prohibited unless prescribed conditions are complied with - Abrievated Graph Key: I16"@en-AU ;
    skos:definition "2 4  Export of prescribed organic goods is prohibited unless prescribed conditions are complied with"@en-AU ;
    skos:narrower F2021L00339:10 ;
    skos:prefLabel "Item I16"@en-AU ;
    dcat:accessURL <https://www.legislation.gov.au/F2021L00339/2023-08-04/2023-08-04/text/original/epub/OEBPS/document_1/document_1.html#_Toc143615153> ;
    dcat:landingPage "https://www.legislation.gov.au/F2021L00339/2023-08-04/2023-08-04/text/original/epub/OEBPS/document_1/document_1.html#_Toc143615153"^^xsd:anyURI ;
    dcat:theme legcons:Item .

F2021L00339:17 a legcons:Part,
        owl:Class,
        dcat:Resource ;
    rdfs:label "Part - P17 Part 2 Exemptions"@en-AU ;
    dct:isPartOf F2021L00339:9 ;
    dct:isReferencedBy F2021L00339: ;
    rdfs:comment "Part 2 Exemptions - Abrievated Graph Key: P17"@en-AU ;
    skos:definition "Part 2 Exemptions"@en-AU ;
    skos:narrower F2021L00339:9 ;
    skos:prefLabel "Part P17"@en-AU ;
    dcat:accessURL <https://www.legislation.gov.au/F2021L00339/2023-08-04/2023-08-04/text/original/epub/OEBPS/document_1/document_1.html#_Toc143615154> ;
    dcat:landingPage "https://www.legislation.gov.au/F2021L00339/2023-08-04/2023-08-04/text/original/epub/OEBPS/document_1/document_1.html#_Toc143615154"^^xsd:anyURI ;
    dcat:theme legcons:Part .

F2021L00339:18 a legcons:Item,
        owl:Class,
        dcat:Resource ;
    rdfs:label "Item - I18 2 5  Application of this Part"@en-AU ;
    dct:isPartOf F2021L00339:9 ;
    dct:isReferencedBy F2021L00339: ;
    rdfs:comment "2 5  Application of this Part - Abrievated Graph Key: I18"@en-AU ;
    skos:definition "2 5  Application of this Part"@en-AU ;
    skos:narrower F2021L00339:9 ;
    skos:prefLabel "Item I18"@en-AU ;
    dcat:accessURL <https://www.legislation.gov.au/F2021L00339/2023-08-04/2023-08-04/text/original/epub/OEBPS/document_1/document_1.html#_Toc143615155> ;
    dcat:landingPage "https://www.legislation.gov.au/F2021L00339/2023-08-04/2023-08-04/text/original/epub/OEBPS/document_1/document_1.html#_Toc143615155"^^xsd:anyURI ;
    dcat:theme legcons:Item .

F2021L00339:19 a legcons:Item,
        owl:Class,
        dcat:Resource ;
    rdfs:label "Item - I19 2 6  Period for making application for exemption"@en-AU ;
    dct:isPartOf F2021L00339:9 ;
    dct:isReferencedBy F2021L00339: ;
    rdfs:comment "2 6  Period for making application for exemption - Abrievated Graph Key: I19"@en-AU ;
    skos:definition "2 6  Period for making application for exemption"@en-AU ;
    skos:narrower F2021L00339:9 ;
    skos:prefLabel "Item I19"@en-AU ;
    dcat:accessURL <https://www.legislation.gov.au/F2021L00339/2023-08-04/2023-08-04/text/original/epub/OEBPS/document_1/document_1.html#_Toc143615156> ;
    dcat:landingPage "https://www.legislation.gov.au/F2021L00339/2023-08-04/2023-08-04/text/original/epub/OEBPS/document_1/document_1.html#_Toc143615156"^^xsd:anyURI ;
    dcat:theme legcons:Item .

F2021L00339:2 a legcons:Part,
        owl:Class,
        dcat:Resource ;
    rdfs:label "Part - P2 Part 1 Preliminary"@en-AU ;
    dct:isPartOf F2021L00339:1 ;
    dct:isReferencedBy F2021L00339: ;
    rdfs:comment "Part 1 Preliminary - Abrievated Graph Key: P2"@en-AU ;
    skos:definition "Part 1 Preliminary"@en-AU ;
    skos:narrower F2021L00339:1 ;
    skos:prefLabel "Part P2"@en-AU ;
    dcat:accessURL <https://www.legislation.gov.au/F2021L00339/2023-08-04/2023-08-04/text/original/epub/OEBPS/document_1/document_1.html#_Toc143615139> ;
    dcat:landingPage "https://www.legislation.gov.au/F2021L00339/2023-08-04/2023-08-04/text/original/epub/OEBPS/document_1/document_1.html#_Toc143615139"^^xsd:anyURI ;
    dcat:theme legcons:Part .

F2021L00339:20 a legcons:Item,
        owl:Class,
        dcat:Resource ;
    rdfs:label "Item - I20 2 7  Conditions of exemptionmatters to which Secretary must have regard"@en-AU ;
    dct:isPartOf F2021L00339:9 ;
    dct:isReferencedBy F2021L00339: ;
    rdfs:comment "2 7  Conditions of exemptionmatters to which Secretary must have regard - Abrievated Graph Key: I20"@en-AU ;
    skos:definition "2 7  Conditions of exemptionmatters to which Secretary must have regard"@en-AU ;
    skos:narrower F2021L00339:9 ;
    skos:prefLabel "Item I20"@en-AU ;
    dcat:accessURL <https://www.legislation.gov.au/F2021L00339/2023-08-04/2023-08-04/text/original/epub/OEBPS/document_1/document_1.html#_Toc143615157> ;
    dcat:landingPage "https://www.legislation.gov.au/F2021L00339/2023-08-04/2023-08-04/text/original/epub/OEBPS/document_1/document_1.html#_Toc143615157"^^xsd:anyURI ;
    dcat:theme legcons:Item .

F2021L00339:21 a legcons:Item,
        owl:Class,
        dcat:Resource ;
    rdfs:label "Item - I21 2 8  Period of effect of exemption"@en-AU ;
    dct:isPartOf F2021L00339:9 ;
    dct:isReferencedBy F2021L00339: ;
    rdfs:comment "2 8  Period of effect of exemption - Abrievated Graph Key: I21"@en-AU ;
    skos:definition "2 8  Period of effect of exemption"@en-AU ;
    skos:narrower F2021L00339:9 ;
    skos:prefLabel "Item I21"@en-AU ;
    dcat:accessURL <https://www.legislation.gov.au/F2021L00339/2023-08-04/2023-08-04/text/original/epub/OEBPS/document_1/document_1.html#_Toc143615158> ;
    dcat:landingPage "https://www.legislation.gov.au/F2021L00339/2023-08-04/2023-08-04/text/original/epub/OEBPS/document_1/document_1.html#_Toc143615158"^^xsd:anyURI ;
    dcat:theme legcons:Item .

F2021L00339:22 a legcons:Item,
        owl:Class,
        dcat:Resource ;
    rdfs:label "Item - I22 2 9  Variation of conditions of exemptionmatters to which Secretary must have regard"@en-AU ;
    dct:isPartOf F2021L00339:9 ;
    dct:isReferencedBy F2021L00339: ;
    rdfs:comment "2 9  Variation of conditions of exemptionmatters to which Secretary must have regard - Abrievated Graph Key: I22"@en-AU ;
    skos:definition "2 9  Variation of conditions of exemptionmatters to which Secretary must have regard"@en-AU ;
    skos:narrower F2021L00339:9 ;
    skos:prefLabel "Item I22"@en-AU ;
    dcat:accessURL <https://www.legislation.gov.au/F2021L00339/2023-08-04/2023-08-04/text/original/epub/OEBPS/document_1/document_1.html#_Toc143615159> ;
    dcat:landingPage "https://www.legislation.gov.au/F2021L00339/2023-08-04/2023-08-04/text/original/epub/OEBPS/document_1/document_1.html#_Toc143615159"^^xsd:anyURI ;
    dcat:theme legcons:Item .

F2021L00339:23 a legcons:Item,
        owl:Class,
        dcat:Resource ;
    rdfs:label "Item - I23 2 10  Revocation of exemptionmatters to which Secretary must have regard"@en-AU ;
    dct:isPartOf F2021L00339:9 ;
    dct:isReferencedBy F2021L00339: ;
    rdfs:comment "2 10  Revocation of exemptionmatters to which Secretary must have regard - Abrievated Graph Key: I23"@en-AU ;
    skos:definition "2 10  Revocation of exemptionmatters to which Secretary must have regard"@en-AU ;
    skos:narrower F2021L00339:9 ;
    skos:prefLabel "Item I23"@en-AU ;
    dcat:accessURL <https://www.legislation.gov.au/F2021L00339/2023-08-04/2023-08-04/text/original/epub/OEBPS/document_1/document_1.html#_Toc143615160> ;
    dcat:landingPage "https://www.legislation.gov.au/F2021L00339/2023-08-04/2023-08-04/text/original/epub/OEBPS/document_1/document_1.html#_Toc143615160"^^xsd:anyURI ;
    dcat:theme legcons:Item .

F2021L00339:24 a legcons:Part,
        owl:Class,
        dcat:Resource ;
    rdfs:label "Part - P24 Part 3 Organic goods certificates"@en-AU ;
    dct:isPartOf F2021L00339:9 ;
    dct:isReferencedBy F2021L00339: ;
    rdfs:comment "Part 3 Organic goods certificates - Abrievated Graph Key: P24"@en-AU ;
    skos:definition "Part 3 Organic goods certificates"@en-AU ;
    skos:narrower F2021L00339:9 ;
    skos:prefLabel "Part P24"@en-AU ;
    dcat:accessURL <https://www.legislation.gov.au/F2021L00339/2023-08-04/2023-08-04/text/original/epub/OEBPS/document_1/document_1.html#_Toc143615161> ;
    dcat:landingPage "https://www.legislation.gov.au/F2021L00339/2023-08-04/2023-08-04/text/original/epub/OEBPS/document_1/document_1.html#_Toc143615161"^^xsd:anyURI ;
    dcat:theme legcons:Part .

F2021L00339:25 a legcons:Item,
        owl:Class,
        dcat:Resource ;
    rdfs:label "Item - I25 2 11  When organic goods certificate may be issued"@en-AU ;
    dct:isPartOf F2021L00339:9 ;
    dct:isReferencedBy F2021L00339: ;
    rdfs:comment "2 11  When organic goods certificate may be issued - Abrievated Graph Key: I25"@en-AU ;
    skos:definition "2 11  When organic goods certificate may be issued"@en-AU ;
    skos:narrower F2021L00339:9 ;
    skos:prefLabel "Item I25"@en-AU ;
    dcat:accessURL <https://www.legislation.gov.au/F2021L00339/2023-08-04/2023-08-04/text/original/epub/OEBPS/document_1/document_1.html#_Toc143615162> ;
    dcat:landingPage "https://www.legislation.gov.au/F2021L00339/2023-08-04/2023-08-04/text/original/epub/OEBPS/document_1/document_1.html#_Toc143615162"^^xsd:anyURI ;
    dcat:theme legcons:Item .

F2021L00339:26 a legcons:Item,
        owl:Class,
        dcat:Resource ;
    rdfs:label "Item - I26 2 12  Information to be included in organic goods certificate"@en-AU ;
    dct:isPartOf F2021L00339:9 ;
    dct:isReferencedBy F2021L00339: ;
    rdfs:comment "2 12  Information to be included in organic goods certificate - Abrievated Graph Key: I26"@en-AU ;
    skos:definition "2 12  Information to be included in organic goods certificate"@en-AU ;
    skos:narrower F2021L00339:9 ;
    skos:prefLabel "Item I26"@en-AU ;
    dcat:accessURL <https://www.legislation.gov.au/F2021L00339/2023-08-04/2023-08-04/text/original/epub/OEBPS/document_1/document_1.html#_Toc143615163> ;
    dcat:landingPage "https://www.legislation.gov.au/F2021L00339/2023-08-04/2023-08-04/text/original/epub/OEBPS/document_1/document_1.html#_Toc143615163"^^xsd:anyURI ;
    dcat:theme legcons:Item .

F2021L00339:27 a legcons:Item,
        owl:Class,
        dcat:Resource ;
    rdfs:label "Item - I27 2 13  Requirements before organic goods certificate may be issued"@en-AU ;
    dct:isPartOf F2021L00339:9 ;
    dct:isReferencedBy F2021L00339: ;
    rdfs:comment "2 13  Requirements before organic goods certificate may be issued - Abrievated Graph Key: I27"@en-AU ;
    skos:definition "2 13  Requirements before organic goods certificate may be issued"@en-AU ;
    skos:narrower F2021L00339:9 ;
    skos:prefLabel "Item I27"@en-AU ;
    dcat:accessURL <https://www.legislation.gov.au/F2021L00339/2023-08-04/2023-08-04/text/original/epub/OEBPS/document_1/document_1.html#_Toc143615164> ;
    dcat:landingPage "https://www.legislation.gov.au/F2021L00339/2023-08-04/2023-08-04/text/original/epub/OEBPS/document_1/document_1.html#_Toc143615164"^^xsd:anyURI ;
    dcat:theme legcons:Item .

F2021L00339:28 a legcons:Item,
        owl:Class,
        dcat:Resource ;
    rdfs:label "Item - I28 2 14  Issuing bodies for organic goods certificates"@en-AU ;
    dct:isPartOf F2021L00339:9 ;
    dct:isReferencedBy F2021L00339: ;
    rdfs:comment "2 14  Issuing bodies for organic goods certificates - Abrievated Graph Key: I28"@en-AU ;
    skos:definition "2 14  Issuing bodies for organic goods certificates"@en-AU ;
    skos:narrower F2021L00339:9 ;
    skos:prefLabel "Item I28"@en-AU ;
    dcat:accessURL <https://www.legislation.gov.au/F2021L00339/2023-08-04/2023-08-04/text/original/epub/OEBPS/document_1/document_1.html#_Toc143615165> ;
    dcat:landingPage "https://www.legislation.gov.au/F2021L00339/2023-08-04/2023-08-04/text/original/epub/OEBPS/document_1/document_1.html#_Toc143615165"^^xsd:anyURI ;
    dcat:theme legcons:Item .

F2021L00339:29 a legcons:Item,
        owl:Class,
        dcat:Resource ;
    rdfs:label "Item - I29 2 15  Changes that require applicant to give additional or corrected information to issuing body"@en-AU ;
    dct:isPartOf F2021L00339:9 ;
    dct:isReferencedBy F2021L00339: ;
    rdfs:comment "2 15  Changes that require applicant to give additional or corrected information to issuing body - Abrievated Graph Key: I29"@en-AU ;
    skos:definition "2 15  Changes that require applicant to give additional or corrected information to issuing body"@en-AU ;
    skos:narrower F2021L00339:9 ;
    skos:prefLabel "Item I29"@en-AU ;
    dcat:accessURL <https://www.legislation.gov.au/F2021L00339/2023-08-04/2023-08-04/text/original/epub/OEBPS/document_1/document_1.html#_Toc143615166> ;
    dcat:landingPage "https://www.legislation.gov.au/F2021L00339/2023-08-04/2023-08-04/text/original/epub/OEBPS/document_1/document_1.html#_Toc143615166"^^xsd:anyURI ;
    dcat:theme legcons:Item .

F2021L00339:3 a legcons:Item,
        owl:Class,
        dcat:Resource ;
    rdfs:label "Item - I3 1 1  Name"@en-AU ;
    dct:isPartOf F2021L00339:1 ;
    dct:isReferencedBy F2021L00339: ;
    rdfs:comment "1 1  Name - Abrievated Graph Key: I3"@en-AU ;
    skos:definition "1 1  Name"@en-AU ;
    skos:narrower F2021L00339:1 ;
    skos:prefLabel "Item I3"@en-AU ;
    dcat:accessURL <https://www.legislation.gov.au/F2021L00339/2023-08-04/2023-08-04/text/original/epub/OEBPS/document_1/document_1.html#_Toc143615140> ;
    dcat:landingPage "https://www.legislation.gov.au/F2021L00339/2023-08-04/2023-08-04/text/original/epub/OEBPS/document_1/document_1.html#_Toc143615140"^^xsd:anyURI ;
    dcat:theme legcons:Item .

F2021L00339:30 a legcons:Item,
        owl:Class,
        dcat:Resource ;
    rdfs:label "Item - I30 2 16  Circumstances for refusing to issue organic goods certificate"@en-AU ;
    dct:isPartOf F2021L00339:9 ;
    dct:isReferencedBy F2021L00339: ;
    rdfs:comment "2 16  Circumstances for refusing to issue organic goods certificate - Abrievated Graph Key: I30"@en-AU ;
    skos:definition "2 16  Circumstances for refusing to issue organic goods certificate"@en-AU ;
    skos:narrower F2021L00339:9 ;
    skos:prefLabel "Item I30"@en-AU ;
    dcat:accessURL <https://www.legislation.gov.au/F2021L00339/2023-08-04/2023-08-04/text/original/epub/OEBPS/document_1/document_1.html#_Toc143615167> ;
    dcat:landingPage "https://www.legislation.gov.au/F2021L00339/2023-08-04/2023-08-04/text/original/epub/OEBPS/document_1/document_1.html#_Toc143615167"^^xsd:anyURI ;
    dcat:theme legcons:Item .

F2021L00339:31 a legcons:Item,
        owl:Class,
        dcat:Resource ;
    rdfs:label "Item - I31 2 17  Changes that require holder of organic goods certificate to give additional or corrected information to issuing body"@en-AU ;
    dct:isPartOf F2021L00339:9 ;
    dct:isReferencedBy F2021L00339: ;
    rdfs:comment "2 17  Changes that require holder of organic goods certificate to give additional or corrected information to issuing body - Abrievated Graph Key: I31"@en-AU ;
    skos:definition "2 17  Changes that require holder of organic goods certificate to give additional or corrected information to issuing body"@en-AU ;
    skos:narrower F2021L00339:9 ;
    skos:prefLabel "Item I31"@en-AU ;
    dcat:accessURL <https://www.legislation.gov.au/F2021L00339/2023-08-04/2023-08-04/text/original/epub/OEBPS/document_1/document_1.html#_Toc143615168> ;
    dcat:landingPage "https://www.legislation.gov.au/F2021L00339/2023-08-04/2023-08-04/text/original/epub/OEBPS/document_1/document_1.html#_Toc143615168"^^xsd:anyURI ;
    dcat:theme legcons:Item .

F2021L00339:32 a legcons:Item,
        owl:Class,
        dcat:Resource ;
    rdfs:label "Item - I32 2 18  Circumstances for revoking organic goods certificate"@en-AU ;
    dct:isPartOf F2021L00339:9 ;
    dct:isReferencedBy F2021L00339: ;
    rdfs:comment "2 18  Circumstances for revoking organic goods certificate - Abrievated Graph Key: I32"@en-AU ;
    skos:definition "2 18  Circumstances for revoking organic goods certificate"@en-AU ;
    skos:narrower F2021L00339:9 ;
    skos:prefLabel "Item I32"@en-AU ;
    dcat:accessURL <https://www.legislation.gov.au/F2021L00339/2023-08-04/2023-08-04/text/original/epub/OEBPS/document_1/document_1.html#_Toc143615169> ;
    dcat:landingPage "https://www.legislation.gov.au/F2021L00339/2023-08-04/2023-08-04/text/original/epub/OEBPS/document_1/document_1.html#_Toc143615169"^^xsd:anyURI ;
    dcat:theme legcons:Item .

F2021L00339:33 a legcons:Item,
        owl:Class,
        dcat:Resource ;
    rdfs:label "Item - I33 2 19  Return of organic goods certificate"@en-AU ;
    dct:isPartOf F2021L00339:9 ;
    dct:isReferencedBy F2021L00339: ;
    rdfs:comment "2 19  Return of organic goods certificate - Abrievated Graph Key: I33"@en-AU ;
    skos:definition "2 19  Return of organic goods certificate"@en-AU ;
    skos:narrower F2021L00339:9 ;
    skos:prefLabel "Item I33"@en-AU ;
    dcat:accessURL <https://www.legislation.gov.au/F2021L00339/2023-08-04/2023-08-04/text/original/epub/OEBPS/document_1/document_1.html#_Toc143615170> ;
    dcat:landingPage "https://www.legislation.gov.au/F2021L00339/2023-08-04/2023-08-04/text/original/epub/OEBPS/document_1/document_1.html#_Toc143615170"^^xsd:anyURI ;
    dcat:theme legcons:Item .

F2021L00339:36 a legcons:Item,
        owl:Class,
        dcat:Resource ;
    rdfs:label "Item - I36 5 1  Proposed arrangement for organic goods certification operations"@en-AU ;
    dct:isPartOf F2021L00339:35 ;
    dct:isReferencedBy F2021L00339: ;
    rdfs:comment "5 1  Proposed arrangement for organic goods certification operations - Abrievated Graph Key: I36"@en-AU ;
    skos:definition "5 1  Proposed arrangement for organic goods certification operations"@en-AU ;
    skos:narrower F2021L00339:35 ;
    skos:prefLabel "Item I36"@en-AU ;
    dcat:accessURL <https://www.legislation.gov.au/F2021L00339/2023-08-04/2023-08-04/text/original/epub/OEBPS/document_1/document_1.html#_Toc143615173> ;
    dcat:landingPage "https://www.legislation.gov.au/F2021L00339/2023-08-04/2023-08-04/text/original/epub/OEBPS/document_1/document_1.html#_Toc143615173"^^xsd:anyURI ;
    dcat:theme legcons:Item .

F2021L00339:39 a legcons:Item,
        owl:Class,
        dcat:Resource ;
    rdfs:label "Item - I39 5 2  Purpose of this Part"@en-AU ;
    dct:isPartOf F2021L00339:38 ;
    dct:isReferencedBy F2021L00339: ;
    rdfs:comment "5 2  Purpose of this Part - Abrievated Graph Key: I39"@en-AU ;
    skos:definition "5 2  Purpose of this Part"@en-AU ;
    skos:narrower F2021L00339:38 ;
    skos:prefLabel "Item I39"@en-AU ;
    dcat:accessURL <https://www.legislation.gov.au/F2021L00339/2023-08-04/2023-08-04/text/original/epub/OEBPS/document_1/document_1.html#_Toc143615176> ;
    dcat:landingPage "https://www.legislation.gov.au/F2021L00339/2023-08-04/2023-08-04/text/original/epub/OEBPS/document_1/document_1.html#_Toc143615176"^^xsd:anyURI ;
    dcat:theme legcons:Item .

F2021L00339:4 a legcons:Item,
        owl:Class,
        dcat:Resource ;
    rdfs:label "Item - I4 1 3  Authority"@en-AU ;
    dct:isPartOf F2021L00339:1 ;
    dct:isReferencedBy F2021L00339: ;
    rdfs:comment "1 3  Authority - Abrievated Graph Key: I4"@en-AU ;
    skos:definition "1 3  Authority"@en-AU ;
    skos:narrower F2021L00339:1 ;
    skos:prefLabel "Item I4"@en-AU ;
    dcat:accessURL <https://www.legislation.gov.au/F2021L00339/2023-08-04/2023-08-04/text/original/epub/OEBPS/document_1/document_1.html#_Toc143615141> ;
    dcat:landingPage "https://www.legislation.gov.au/F2021L00339/2023-08-04/2023-08-04/text/original/epub/OEBPS/document_1/document_1.html#_Toc143615141"^^xsd:anyURI ;
    dcat:theme legcons:Item .

F2021L00339:41 a legcons:Item,
        owl:Class,
        dcat:Resource ;
    rdfs:label "Item - I41 5 3  Requirements of National Organic Standard must be met"@en-AU ;
    dct:isPartOf F2021L00339:40 ;
    dct:isReferencedBy F2021L00339: ;
    rdfs:comment "5 3  Requirements of National Organic Standard must be met - Abrievated Graph Key: I41"@en-AU ;
    skos:definition "5 3  Requirements of National Organic Standard must be met"@en-AU ;
    skos:narrower F2021L00339:40 ;
    skos:prefLabel "Item I41"@en-AU ;
    dcat:accessURL <https://www.legislation.gov.au/F2021L00339/2023-08-04/2023-08-04/text/original/epub/OEBPS/document_1/document_1.html#_Toc143615178> ;
    dcat:landingPage "https://www.legislation.gov.au/F2021L00339/2023-08-04/2023-08-04/text/original/epub/OEBPS/document_1/document_1.html#_Toc143615178"^^xsd:anyURI ;
    dcat:theme legcons:Item .

F2021L00339:42 a legcons:Item,
        owl:Class,
        dcat:Resource ;
    rdfs:label "Item - I42 5 4  Importing country requirements must be met"@en-AU ;
    dct:isPartOf F2021L00339:40 ;
    dct:isReferencedBy F2021L00339: ;
    rdfs:comment "5 4  Importing country requirements must be met - Abrievated Graph Key: I42"@en-AU ;
    skos:definition "5 4  Importing country requirements must be met"@en-AU ;
    skos:narrower F2021L00339:40 ;
    skos:prefLabel "Item I42"@en-AU ;
    dcat:accessURL <https://www.legislation.gov.au/F2021L00339/2023-08-04/2023-08-04/text/original/epub/OEBPS/document_1/document_1.html#_Toc143615179> ;
    dcat:landingPage "https://www.legislation.gov.au/F2021L00339/2023-08-04/2023-08-04/text/original/epub/OEBPS/document_1/document_1.html#_Toc143615179"^^xsd:anyURI ;
    dcat:theme legcons:Item .

F2021L00339:43 a legcons:Item,
        owl:Class,
        dcat:Resource ;
    rdfs:label "Item - I43 5 5  Organic goods certificates must be in approved form"@en-AU ;
    dct:isPartOf F2021L00339:40 ;
    dct:isReferencedBy F2021L00339: ;
    rdfs:comment "5 5  Organic goods certificates must be in approved form - Abrievated Graph Key: I43"@en-AU ;
    skos:definition "5 5  Organic goods certificates must be in approved form"@en-AU ;
    skos:narrower F2021L00339:40 ;
    skos:prefLabel "Item I43"@en-AU ;
    dcat:accessURL <https://www.legislation.gov.au/F2021L00339/2023-08-04/2023-08-04/text/original/epub/OEBPS/document_1/document_1.html#_Toc143615180> ;
    dcat:landingPage "https://www.legislation.gov.au/F2021L00339/2023-08-04/2023-08-04/text/original/epub/OEBPS/document_1/document_1.html#_Toc143615180"^^xsd:anyURI ;
    dcat:theme legcons:Item .

F2021L00339:45 a legcons:Item,
        owl:Class,
        dcat:Resource ;
    rdfs:label "Item - I45 5 6  Operations must be objective fair etc"@en-AU ;
    dct:isPartOf F2021L00339:44 ;
    dct:isReferencedBy F2021L00339: ;
    rdfs:comment "5 6  Operations must be objective fair etc - Abrievated Graph Key: I45"@en-AU ;
    skos:definition "5 6  Operations must be objective fair etc"@en-AU ;
    skos:narrower F2021L00339:44 ;
    skos:prefLabel "Item I45"@en-AU ;
    dcat:accessURL <https://www.legislation.gov.au/F2021L00339/2023-08-04/2023-08-04/text/original/epub/OEBPS/document_1/document_1.html#_Toc143615182> ;
    dcat:landingPage "https://www.legislation.gov.au/F2021L00339/2023-08-04/2023-08-04/text/original/epub/OEBPS/document_1/document_1.html#_Toc143615182"^^xsd:anyURI ;
    dcat:theme legcons:Item .

F2021L00339:46 a legcons:Item,
        owl:Class,
        dcat:Resource ;
    rdfs:label "Item - I46 5 7  Management practices organisational structure resources and personnel"@en-AU ;
    dct:isPartOf F2021L00339:44 ;
    dct:isReferencedBy F2021L00339: ;
    rdfs:comment "5 7  Management practices organisational structure resources and personnel - Abrievated Graph Key: I46"@en-AU ;
    skos:definition "5 7  Management practices organisational structure resources and personnel"@en-AU ;
    skos:narrower F2021L00339:44 ;
    skos:prefLabel "Item I46"@en-AU ;
    dcat:accessURL <https://www.legislation.gov.au/F2021L00339/2023-08-04/2023-08-04/text/original/epub/OEBPS/document_1/document_1.html#_Toc143615183> ;
    dcat:landingPage "https://www.legislation.gov.au/F2021L00339/2023-08-04/2023-08-04/text/original/epub/OEBPS/document_1/document_1.html#_Toc143615183"^^xsd:anyURI ;
    dcat:theme legcons:Item .

F2021L00339:47 a legcons:Item,
        owl:Class,
        dcat:Resource ;
    rdfs:label "Item - I47 5 8  Verification of compliance with the Act and other matters"@en-AU ;
    dct:isPartOf F2021L00339:44 ;
    dct:isReferencedBy F2021L00339: ;
    rdfs:comment "5 8  Verification of compliance with the Act and other matters - Abrievated Graph Key: I47"@en-AU ;
    skos:definition "5 8  Verification of compliance with the Act and other matters"@en-AU ;
    skos:narrower F2021L00339:44 ;
    skos:prefLabel "Item I47"@en-AU ;
    dcat:accessURL <https://www.legislation.gov.au/F2021L00339/2023-08-04/2023-08-04/text/original/epub/OEBPS/document_1/document_1.html#_Toc143615184> ;
    dcat:landingPage "https://www.legislation.gov.au/F2021L00339/2023-08-04/2023-08-04/text/original/epub/OEBPS/document_1/document_1.html#_Toc143615184"^^xsd:anyURI ;
    dcat:theme legcons:Item .

F2021L00339:48 a legcons:Item,
        owl:Class,
        dcat:Resource ;
    rdfs:label "Item - I48 5 9  Action must be taken to address non compliance"@en-AU ;
    dct:isPartOf F2021L00339:44 ;
    dct:isReferencedBy F2021L00339: ;
    rdfs:comment "5 9  Action must be taken to address non compliance - Abrievated Graph Key: I48"@en-AU ;
    skos:definition "5 9  Action must be taken to address non compliance"@en-AU ;
    skos:narrower F2021L00339:44 ;
    skos:prefLabel "Item I48"@en-AU ;
    dcat:accessURL <https://www.legislation.gov.au/F2021L00339/2023-08-04/2023-08-04/text/original/epub/OEBPS/document_1/document_1.html#_Toc143615185> ;
    dcat:landingPage "https://www.legislation.gov.au/F2021L00339/2023-08-04/2023-08-04/text/original/epub/OEBPS/document_1/document_1.html#_Toc143615185"^^xsd:anyURI ;
    dcat:theme legcons:Item .

F2021L00339:49 a legcons:Item,
        owl:Class,
        dcat:Resource ;
    rdfs:label "Item - I49 5 10  Internal audit and management review"@en-AU ;
    dct:isPartOf F2021L00339:44 ;
    dct:isReferencedBy F2021L00339: ;
    rdfs:comment "5 10  Internal audit and management review - Abrievated Graph Key: I49"@en-AU ;
    skos:definition "5 10  Internal audit and management review"@en-AU ;
    skos:narrower F2021L00339:44 ;
    skos:prefLabel "Item I49"@en-AU ;
    dcat:accessURL <https://www.legislation.gov.au/F2021L00339/2023-08-04/2023-08-04/text/original/epub/OEBPS/document_1/document_1.html#_Toc143615186> ;
    dcat:landingPage "https://www.legislation.gov.au/F2021L00339/2023-08-04/2023-08-04/text/original/epub/OEBPS/document_1/document_1.html#_Toc143615186"^^xsd:anyURI ;
    dcat:theme legcons:Item .

F2021L00339:5 a legcons:Item,
        owl:Class,
        dcat:Resource ;
    rdfs:label "Item - I5 1 4  Application of this instrument"@en-AU ;
    dct:isPartOf F2021L00339:1 ;
    dct:isReferencedBy F2021L00339: ;
    rdfs:comment "1 4  Application of this instrument - Abrievated Graph Key: I5"@en-AU ;
    skos:definition "1 4  Application of this instrument"@en-AU ;
    skos:narrower F2021L00339:1 ;
    skos:prefLabel "Item I5"@en-AU ;
    dcat:accessURL <https://www.legislation.gov.au/F2021L00339/2023-08-04/2023-08-04/text/original/epub/OEBPS/document_1/document_1.html#_Toc143615142> ;
    dcat:landingPage "https://www.legislation.gov.au/F2021L00339/2023-08-04/2023-08-04/text/original/epub/OEBPS/document_1/document_1.html#_Toc143615142"^^xsd:anyURI ;
    dcat:theme legcons:Item .

F2021L00339:50 a legcons:Item,
        owl:Class,
        dcat:Resource ;
    rdfs:label "Item - I50 5 11  Secretary must be notified of critical non compliance"@en-AU ;
    dct:isPartOf F2021L00339:44 ;
    dct:isReferencedBy F2021L00339: ;
    rdfs:comment "5 11  Secretary must be notified of critical non compliance - Abrievated Graph Key: I50"@en-AU ;
    skos:definition "5 11  Secretary must be notified of critical non compliance"@en-AU ;
    skos:narrower F2021L00339:44 ;
    skos:prefLabel "Item I50"@en-AU ;
    dcat:accessURL <https://www.legislation.gov.au/F2021L00339/2023-08-04/2023-08-04/text/original/epub/OEBPS/document_1/document_1.html#_Toc143615187> ;
    dcat:landingPage "https://www.legislation.gov.au/F2021L00339/2023-08-04/2023-08-04/text/original/epub/OEBPS/document_1/document_1.html#_Toc143615187"^^xsd:anyURI ;
    dcat:theme legcons:Item .

F2021L00339:52 a legcons:Item,
        owl:Class,
        dcat:Resource ;
    rdfs:label "Item - I52 5 12  Period within which application to renew approved arrangement must be made"@en-AU ;
    dct:isPartOf F2021L00339:51 ;
    dct:isReferencedBy F2021L00339: ;
    rdfs:comment "5 12  Period within which application to renew approved arrangement must be made - Abrievated Graph Key: I52"@en-AU ;
    skos:definition "5 12  Period within which application to renew approved arrangement must be made"@en-AU ;
    skos:narrower F2021L00339:51 ;
    skos:prefLabel "Item I52"@en-AU ;
    dcat:accessURL <https://www.legislation.gov.au/F2021L00339/2023-08-04/2023-08-04/text/original/epub/OEBPS/document_1/document_1.html#_Toc143615189> ;
    dcat:landingPage "https://www.legislation.gov.au/F2021L00339/2023-08-04/2023-08-04/text/original/epub/OEBPS/document_1/document_1.html#_Toc143615189"^^xsd:anyURI ;
    dcat:theme legcons:Item .

F2021L00339:55 a legcons:Item,
        owl:Class,
        dcat:Resource ;
    rdfs:label "Item - I55 5 13  Significant variations"@en-AU ;
    dct:isPartOf F2021L00339:54 ;
    dct:isReferencedBy F2021L00339: ;
    rdfs:comment "5 13  Significant variations - Abrievated Graph Key: I55"@en-AU ;
    skos:definition "5 13  Significant variations"@en-AU ;
    skos:narrower F2021L00339:54 ;
    skos:prefLabel "Item I55"@en-AU ;
    dcat:accessURL <https://www.legislation.gov.au/F2021L00339/2023-08-04/2023-08-04/text/original/epub/OEBPS/document_1/document_1.html#_Toc143615192> ;
    dcat:landingPage "https://www.legislation.gov.au/F2021L00339/2023-08-04/2023-08-04/text/original/epub/OEBPS/document_1/document_1.html#_Toc143615192"^^xsd:anyURI ;
    dcat:theme legcons:Item .

F2021L00339:57 a legcons:Item,
        owl:Class,
        dcat:Resource ;
    rdfs:label "Item - I57 5 14  Other reasons for requiring holder to vary approved arrangement"@en-AU ;
    dct:isPartOf F2021L00339:56 ;
    dct:isReferencedBy F2021L00339: ;
    rdfs:comment "5 14  Other reasons for requiring holder to vary approved arrangement - Abrievated Graph Key: I57"@en-AU ;
    skos:definition "5 14  Other reasons for requiring holder to vary approved arrangement"@en-AU ;
    skos:narrower F2021L00339:56 ;
    skos:prefLabel "Item I57"@en-AU ;
    dcat:accessURL <https://www.legislation.gov.au/F2021L00339/2023-08-04/2023-08-04/text/original/epub/OEBPS/document_1/document_1.html#_Toc143615194> ;
    dcat:landingPage "https://www.legislation.gov.au/F2021L00339/2023-08-04/2023-08-04/text/original/epub/OEBPS/document_1/document_1.html#_Toc143615194"^^xsd:anyURI ;
    dcat:theme legcons:Item .

F2021L00339:59 a legcons:Item,
        owl:Class,
        dcat:Resource ;
    rdfs:label "Item - I59 5 15  Other events of which Secretary must be notified"@en-AU ;
    dct:isPartOf F2021L00339:58 ;
    dct:isReferencedBy F2021L00339: ;
    rdfs:comment "5 15  Other events of which Secretary must be notified - Abrievated Graph Key: I59"@en-AU ;
    skos:definition "5 15  Other events of which Secretary must be notified"@en-AU ;
    skos:narrower F2021L00339:58 ;
    skos:prefLabel "Item I59"@en-AU ;
    dcat:accessURL <https://www.legislation.gov.au/F2021L00339/2023-08-04/2023-08-04/text/original/epub/OEBPS/document_1/document_1.html#_Toc143615196> ;
    dcat:landingPage "https://www.legislation.gov.au/F2021L00339/2023-08-04/2023-08-04/text/original/epub/OEBPS/document_1/document_1.html#_Toc143615196"^^xsd:anyURI ;
    dcat:theme legcons:Item .

F2021L00339:6 a legcons:Item,
        owl:Class,
        dcat:Resource ;
    rdfs:label "Item - I6 1 5  Simplified outline of this instrument"@en-AU ;
    dct:isPartOf F2021L00339:1 ;
    dct:isReferencedBy F2021L00339: ;
    rdfs:comment "1 5  Simplified outline of this instrument - Abrievated Graph Key: I6"@en-AU ;
    skos:definition "1 5  Simplified outline of this instrument"@en-AU ;
    skos:narrower F2021L00339:1 ;
    skos:prefLabel "Item I6"@en-AU ;
    dcat:accessURL <https://www.legislation.gov.au/F2021L00339/2023-08-04/2023-08-04/text/original/epub/OEBPS/document_1/document_1.html#_Toc143615143> ;
    dcat:landingPage "https://www.legislation.gov.au/F2021L00339/2023-08-04/2023-08-04/text/original/epub/OEBPS/document_1/document_1.html#_Toc143615143"^^xsd:anyURI ;
    dcat:theme legcons:Item .

F2021L00339:61 a legcons:Item,
        owl:Class,
        dcat:Resource ;
    rdfs:label "Item - I61 5 16  Kinds of persons who are required to be fit and proper persons"@en-AU ;
    dct:isPartOf F2021L00339:60 ;
    dct:isReferencedBy F2021L00339: ;
    rdfs:comment "5 16  Kinds of persons who are required to be fit and proper persons - Abrievated Graph Key: I61"@en-AU ;
    skos:definition "5 16  Kinds of persons who are required to be fit and proper persons"@en-AU ;
    skos:narrower F2021L00339:60 ;
    skos:prefLabel "Item I61"@en-AU ;
    dcat:accessURL <https://www.legislation.gov.au/F2021L00339/2023-08-04/2023-08-04/text/original/epub/OEBPS/document_1/document_1.html#_Toc143615198> ;
    dcat:landingPage "https://www.legislation.gov.au/F2021L00339/2023-08-04/2023-08-04/text/original/epub/OEBPS/document_1/document_1.html#_Toc143615198"^^xsd:anyURI ;
    dcat:theme legcons:Item .

F2021L00339:63 a legcons:Item,
        owl:Class,
        dcat:Resource ;
    rdfs:label "Item - I63 5 17  Application of this Part"@en-AU ;
    dct:isPartOf F2021L00339:62 ;
    dct:isReferencedBy F2021L00339: ;
    rdfs:comment "5 17  Application of this Part - Abrievated Graph Key: I63"@en-AU ;
    skos:definition "5 17  Application of this Part"@en-AU ;
    skos:narrower F2021L00339:62 ;
    skos:prefLabel "Item I63"@en-AU ;
    dcat:accessURL <https://www.legislation.gov.au/F2021L00339/2023-08-04/2023-08-04/text/original/epub/OEBPS/document_1/document_1.html#_Toc143615200> ;
    dcat:landingPage "https://www.legislation.gov.au/F2021L00339/2023-08-04/2023-08-04/text/original/epub/OEBPS/document_1/document_1.html#_Toc143615200"^^xsd:anyURI ;
    dcat:theme legcons:Item .

F2021L00339:64 a legcons:Item,
        owl:Class,
        dcat:Resource ;
    rdfs:label "Item - I64 5 18  Initial consideration period"@en-AU ;
    dct:isPartOf F2021L00339:62 ;
    dct:isReferencedBy F2021L00339: ;
    rdfs:comment "5 18  Initial consideration period - Abrievated Graph Key: I64"@en-AU ;
    skos:definition "5 18  Initial consideration period"@en-AU ;
    skos:narrower F2021L00339:62 ;
    skos:prefLabel "Item I64"@en-AU ;
    dcat:accessURL <https://www.legislation.gov.au/F2021L00339/2023-08-04/2023-08-04/text/original/epub/OEBPS/document_1/document_1.html#_Toc143615201> ;
    dcat:landingPage "https://www.legislation.gov.au/F2021L00339/2023-08-04/2023-08-04/text/original/epub/OEBPS/document_1/document_1.html#_Toc143615201"^^xsd:anyURI ;
    dcat:theme legcons:Item .

F2021L00339:65 a legcons:Item,
        owl:Class,
        dcat:Resource ;
    rdfs:label "Item - I65 5 19  Period within which request relating to application must be complied with"@en-AU ;
    dct:isPartOf F2021L00339:62 ;
    dct:isReferencedBy F2021L00339: ;
    rdfs:comment "5 19  Period within which request relating to application must be complied with - Abrievated Graph Key: I65"@en-AU ;
    skos:definition "5 19  Period within which request relating to application must be complied with"@en-AU ;
    skos:narrower F2021L00339:62 ;
    skos:prefLabel "Item I65"@en-AU ;
    dcat:accessURL <https://www.legislation.gov.au/F2021L00339/2023-08-04/2023-08-04/text/original/epub/OEBPS/document_1/document_1.html#_Toc143615202> ;
    dcat:landingPage "https://www.legislation.gov.au/F2021L00339/2023-08-04/2023-08-04/text/original/epub/OEBPS/document_1/document_1.html#_Toc143615202"^^xsd:anyURI ;
    dcat:theme legcons:Item .

F2021L00339:66 a legcons:Chapter,
        owl:Class,
        dcat:Resource ;
    rdfs:label "Chapter - C66 Chapter 8 Other matters relating to export"@en-AU ;
    dct:hasPart F2021L00339:67 ;
    dct:isReferencedBy F2021L00339: ;
    rdfs:comment "Chapter 8 Other matters relating to export - Abrievated Graph Key: C66"@en-AU ;
    skos:broader F2021L00339:67 ;
    skos:definition "Chapter 8 Other matters relating to export"@en-AU ;
    skos:prefLabel "Chapter C66"@en-AU ;
    dcat:accessURL <https://www.legislation.gov.au/F2021L00339/2023-08-04/2023-08-04/text/original/epub/OEBPS/document_1/document_1.html#_Toc143615203> ;
    dcat:landingPage "https://www.legislation.gov.au/F2021L00339/2023-08-04/2023-08-04/text/original/epub/OEBPS/document_1/document_1.html#_Toc143615203"^^xsd:anyURI ;
    dcat:theme legcons:Chapter .

F2021L00339:68 a legcons:Item,
        owl:Class,
        dcat:Resource ;
    rdfs:label "Item - I68 8 1  Purpose of this Part"@en-AU ;
    dct:isPartOf F2021L00339:67 ;
    dct:isReferencedBy F2021L00339: ;
    rdfs:comment "8 1  Purpose of this Part - Abrievated Graph Key: I68"@en-AU ;
    skos:definition "8 1  Purpose of this Part"@en-AU ;
    skos:narrower F2021L00339:67 ;
    skos:prefLabel "Item I68"@en-AU ;
    dcat:accessURL <https://www.legislation.gov.au/F2021L00339/2023-08-04/2023-08-04/text/original/epub/OEBPS/document_1/document_1.html#_Toc143615205> ;
    dcat:landingPage "https://www.legislation.gov.au/F2021L00339/2023-08-04/2023-08-04/text/original/epub/OEBPS/document_1/document_1.html#_Toc143615205"^^xsd:anyURI ;
    dcat:theme legcons:Item .

F2021L00339:69 a legcons:Item,
        owl:Class,
        dcat:Resource ;
    rdfs:label "Item - I69 8 2  Trade description must be applied to prescribed organic goods that are intended to be exported"@en-AU ;
    dct:isPartOf F2021L00339:67 ;
    dct:isReferencedBy F2021L00339: ;
    rdfs:comment "8 2  Trade description must be applied to prescribed organic goods that are intended to be exported - Abrievated Graph Key: I69"@en-AU ;
    skos:definition "8 2  Trade description must be applied to prescribed organic goods that are intended to be exported"@en-AU ;
    skos:narrower F2021L00339:67 ;
    skos:prefLabel "Item I69"@en-AU ;
    dcat:accessURL <https://www.legislation.gov.au/F2021L00339/2023-08-04/2023-08-04/text/original/epub/OEBPS/document_1/document_1.html#_Toc143615206> ;
    dcat:landingPage "https://www.legislation.gov.au/F2021L00339/2023-08-04/2023-08-04/text/original/epub/OEBPS/document_1/document_1.html#_Toc143615206"^^xsd:anyURI ;
    dcat:theme legcons:Item .

F2021L00339:7 a legcons:Part,
        owl:Class,
        dcat:Resource ;
    rdfs:label "Part - P7 Part 2 Interpretation"@en-AU ;
    dct:isPartOf F2021L00339:1 ;
    dct:isReferencedBy F2021L00339: ;
    rdfs:comment "Part 2 Interpretation - Abrievated Graph Key: P7"@en-AU ;
    skos:definition "Part 2 Interpretation"@en-AU ;
    skos:narrower F2021L00339:1 ;
    skos:prefLabel "Part P7"@en-AU ;
    dcat:accessURL <https://www.legislation.gov.au/F2021L00339/2023-08-04/2023-08-04/text/original/epub/OEBPS/document_1/document_1.html#_Toc143615144> ;
    dcat:landingPage "https://www.legislation.gov.au/F2021L00339/2023-08-04/2023-08-04/text/original/epub/OEBPS/document_1/document_1.html#_Toc143615144"^^xsd:anyURI ;
    dcat:theme legcons:Part .

F2021L00339:70 a legcons:Item,
        owl:Class,
        dcat:Resource ;
    rdfs:label "Item - I70 8 3  General requirements for trade descriptions"@en-AU ;
    dct:isPartOf F2021L00339:67 ;
    dct:isReferencedBy F2021L00339: ;
    rdfs:comment "8 3  General requirements for trade descriptions - Abrievated Graph Key: I70"@en-AU ;
    skos:definition "8 3  General requirements for trade descriptions"@en-AU ;
    skos:narrower F2021L00339:67 ;
    skos:prefLabel "Item I70"@en-AU ;
    dcat:accessURL <https://www.legislation.gov.au/F2021L00339/2023-08-04/2023-08-04/text/original/epub/OEBPS/document_1/document_1.html#_Toc143615207> ;
    dcat:landingPage "https://www.legislation.gov.au/F2021L00339/2023-08-04/2023-08-04/text/original/epub/OEBPS/document_1/document_1.html#_Toc143615207"^^xsd:anyURI ;
    dcat:theme legcons:Item .

F2021L00339:71 a legcons:Item,
        owl:Class,
        dcat:Resource ;
    rdfs:label "Item - I71 8 4  Trade descriptions in language other than English"@en-AU ;
    dct:isPartOf F2021L00339:67 ;
    dct:isReferencedBy F2021L00339: ;
    rdfs:comment "8 4  Trade descriptions in language other than English - Abrievated Graph Key: I71"@en-AU ;
    skos:definition "8 4  Trade descriptions in language other than English"@en-AU ;
    skos:narrower F2021L00339:67 ;
    skos:prefLabel "Item I71"@en-AU ;
    dcat:accessURL <https://www.legislation.gov.au/F2021L00339/2023-08-04/2023-08-04/text/original/epub/OEBPS/document_1/document_1.html#_Toc143615208> ;
    dcat:landingPage "https://www.legislation.gov.au/F2021L00339/2023-08-04/2023-08-04/text/original/epub/OEBPS/document_1/document_1.html#_Toc143615208"^^xsd:anyURI ;
    dcat:theme legcons:Item .

F2021L00339:75 a legcons:Item,
        owl:Class,
        dcat:Resource ;
    rdfs:label "Item - I75 9 1  References to audit in this Part"@en-AU ;
    dct:isPartOf F2021L00339:74 ;
    dct:isReferencedBy F2021L00339: ;
    rdfs:comment "9 1  References to audit in this Part - Abrievated Graph Key: I75"@en-AU ;
    skos:definition "9 1  References to audit in this Part"@en-AU ;
    skos:narrower F2021L00339:74 ;
    skos:prefLabel "Item I75"@en-AU ;
    dcat:accessURL <https://www.legislation.gov.au/F2021L00339/2023-08-04/2023-08-04/text/original/epub/OEBPS/document_1/document_1.html#_Toc143615212> ;
    dcat:landingPage "https://www.legislation.gov.au/F2021L00339/2023-08-04/2023-08-04/text/original/epub/OEBPS/document_1/document_1.html#_Toc143615212"^^xsd:anyURI ;
    dcat:theme legcons:Item .

F2021L00339:77 a legcons:Item,
        owl:Class,
        dcat:Resource ;
    rdfs:label "Item - I77 9 2  Purpose of this Division"@en-AU ;
    dct:isPartOf F2021L00339:76 ;
    dct:isReferencedBy F2021L00339: ;
    rdfs:comment "9 2  Purpose of this Division - Abrievated Graph Key: I77"@en-AU ;
    skos:definition "9 2  Purpose of this Division"@en-AU ;
    skos:narrower F2021L00339:76 ;
    skos:prefLabel "Item I77"@en-AU ;
    dcat:accessURL <https://www.legislation.gov.au/F2021L00339/2023-08-04/2023-08-04/text/original/epub/OEBPS/document_1/document_1.html#_Toc143615214> ;
    dcat:landingPage "https://www.legislation.gov.au/F2021L00339/2023-08-04/2023-08-04/text/original/epub/OEBPS/document_1/document_1.html#_Toc143615214"^^xsd:anyURI ;
    dcat:theme legcons:Item .

F2021L00339:78 a legcons:Item,
        owl:Class,
        dcat:Resource ;
    rdfs:label "Item - I78 9 3  Manner in which audit must be conducted"@en-AU ;
    dct:isPartOf F2021L00339:76 ;
    dct:isReferencedBy F2021L00339: ;
    rdfs:comment "9 3  Manner in which audit must be conducted - Abrievated Graph Key: I78"@en-AU ;
    skos:definition "9 3  Manner in which audit must be conducted"@en-AU ;
    skos:narrower F2021L00339:76 ;
    skos:prefLabel "Item I78"@en-AU ;
    dcat:accessURL <https://www.legislation.gov.au/F2021L00339/2023-08-04/2023-08-04/text/original/epub/OEBPS/document_1/document_1.html#_Toc143615215> ;
    dcat:landingPage "https://www.legislation.gov.au/F2021L00339/2023-08-04/2023-08-04/text/original/epub/OEBPS/document_1/document_1.html#_Toc143615215"^^xsd:anyURI ;
    dcat:theme legcons:Item .

F2021L00339:79 a legcons:Item,
        owl:Class,
        dcat:Resource ;
    rdfs:label "Item - I79 9 4  Audit reports"@en-AU ;
    dct:isPartOf F2021L00339:76 ;
    dct:isReferencedBy F2021L00339: ;
    rdfs:comment "9 4  Audit reports - Abrievated Graph Key: I79"@en-AU ;
    skos:definition "9 4  Audit reports"@en-AU ;
    skos:narrower F2021L00339:76 ;
    skos:prefLabel "Item I79"@en-AU ;
    dcat:accessURL <https://www.legislation.gov.au/F2021L00339/2023-08-04/2023-08-04/text/original/epub/OEBPS/document_1/document_1.html#_Toc143615216> ;
    dcat:landingPage "https://www.legislation.gov.au/F2021L00339/2023-08-04/2023-08-04/text/original/epub/OEBPS/document_1/document_1.html#_Toc143615216"^^xsd:anyURI ;
    dcat:theme legcons:Item .

F2021L00339:8 a legcons:Item,
        owl:Class,
        dcat:Resource ;
    rdfs:label "Item - I8 1 6  Definitions"@en-AU ;
    dct:isPartOf F2021L00339:1 ;
    dct:isReferencedBy F2021L00339: ;
    rdfs:comment "1 6  Definitions - Abrievated Graph Key: I8"@en-AU ;
    skos:definition "1 6  Definitions"@en-AU ;
    skos:narrower F2021L00339:1 ;
    skos:prefLabel "Item I8"@en-AU ;
    dcat:accessURL <https://www.legislation.gov.au/F2021L00339/2023-08-04/2023-08-04/text/original/epub/OEBPS/document_1/document_1.html#_Toc143615145> ;
    dcat:landingPage "https://www.legislation.gov.au/F2021L00339/2023-08-04/2023-08-04/text/original/epub/OEBPS/document_1/document_1.html#_Toc143615145"^^xsd:anyURI ;
    dcat:theme legcons:Item .

F2021L00339:81 a legcons:Item,
        owl:Class,
        dcat:Resource ;
    rdfs:label "Item - I81 9 5  Other grounds for giving direction to relevant person"@en-AU ;
    dct:isPartOf F2021L00339:80 ;
    dct:isReferencedBy F2021L00339: ;
    rdfs:comment "9 5  Other grounds for giving direction to relevant person - Abrievated Graph Key: I81"@en-AU ;
    skos:definition "9 5  Other grounds for giving direction to relevant person"@en-AU ;
    skos:narrower F2021L00339:80 ;
    skos:prefLabel "Item I81"@en-AU ;
    dcat:accessURL <https://www.legislation.gov.au/F2021L00339/2023-08-04/2023-08-04/text/original/epub/OEBPS/document_1/document_1.html#_Toc143615218> ;
    dcat:landingPage "https://www.legislation.gov.au/F2021L00339/2023-08-04/2023-08-04/text/original/epub/OEBPS/document_1/document_1.html#_Toc143615218"^^xsd:anyURI ;
    dcat:theme legcons:Item .

F2021L00339:83 a legcons:Item,
        owl:Class,
        dcat:Resource ;
    rdfs:label "Item - I83 10 1  Samples taken in exercising monitoring or investigation powers"@en-AU ;
    dct:isPartOf F2021L00339:82 ;
    dct:isReferencedBy F2021L00339: ;
    rdfs:comment "10 1  Samples taken in exercising monitoring or investigation powers - Abrievated Graph Key: I83"@en-AU ;
    skos:definition "10 1  Samples taken in exercising monitoring or investigation powers"@en-AU ;
    skos:narrower F2021L00339:82 ;
    skos:prefLabel "Item I83"@en-AU ;
    dcat:accessURL <https://www.legislation.gov.au/F2021L00339/2023-08-04/2023-08-04/text/original/epub/OEBPS/document_1/document_1.html#_Toc143615220> ;
    dcat:landingPage "https://www.legislation.gov.au/F2021L00339/2023-08-04/2023-08-04/text/original/epub/OEBPS/document_1/document_1.html#_Toc143615220"^^xsd:anyURI ;
    dcat:theme legcons:Item .

F2021L00339:84 a legcons:Item,
        owl:Class,
        dcat:Resource ;
    rdfs:label "Item - I84 10 2  Dealing with things seized in exercising investigation powers"@en-AU ;
    dct:isPartOf F2021L00339:82 ;
    dct:isReferencedBy F2021L00339: ;
    rdfs:comment "10 2  Dealing with things seized in exercising investigation powers - Abrievated Graph Key: I84"@en-AU ;
    skos:definition "10 2  Dealing with things seized in exercising investigation powers"@en-AU ;
    skos:narrower F2021L00339:82 ;
    skos:prefLabel "Item I84"@en-AU ;
    dcat:accessURL <https://www.legislation.gov.au/F2021L00339/2023-08-04/2023-08-04/text/original/epub/OEBPS/document_1/document_1.html#_Toc143615221> ;
    dcat:landingPage "https://www.legislation.gov.au/F2021L00339/2023-08-04/2023-08-04/text/original/epub/OEBPS/document_1/document_1.html#_Toc143615221"^^xsd:anyURI ;
    dcat:theme legcons:Item .

F2021L00339:87 a legcons:Item,
        owl:Class,
        dcat:Resource ;
    rdfs:label "Item - I87 11 1  Purpose of this Part"@en-AU ;
    dct:isPartOf F2021L00339:86 ;
    dct:isReferencedBy F2021L00339: ;
    rdfs:comment "11 1  Purpose of this Part - Abrievated Graph Key: I87"@en-AU ;
    skos:definition "11 1  Purpose of this Part"@en-AU ;
    skos:narrower F2021L00339:86 ;
    skos:prefLabel "Item I87"@en-AU ;
    dcat:accessURL <https://www.legislation.gov.au/F2021L00339/2023-08-04/2023-08-04/text/original/epub/OEBPS/document_1/document_1.html#_Toc143615224> ;
    dcat:landingPage "https://www.legislation.gov.au/F2021L00339/2023-08-04/2023-08-04/text/original/epub/OEBPS/document_1/document_1.html#_Toc143615224"^^xsd:anyURI ;
    dcat:theme legcons:Item .

F2021L00339:88 a legcons:Item,
        owl:Class,
        dcat:Resource ;
    rdfs:label "Item - I88 11 2  General requirements for records"@en-AU ;
    dct:isPartOf F2021L00339:86 ;
    dct:isReferencedBy F2021L00339: ;
    rdfs:comment "11 2  General requirements for records - Abrievated Graph Key: I88"@en-AU ;
    skos:definition "11 2  General requirements for records"@en-AU ;
    skos:narrower F2021L00339:86 ;
    skos:prefLabel "Item I88"@en-AU ;
    dcat:accessURL <https://www.legislation.gov.au/F2021L00339/2023-08-04/2023-08-04/text/original/epub/OEBPS/document_1/document_1.html#_Toc143615225> ;
    dcat:landingPage "https://www.legislation.gov.au/F2021L00339/2023-08-04/2023-08-04/text/original/epub/OEBPS/document_1/document_1.html#_Toc143615225"^^xsd:anyURI ;
    dcat:theme legcons:Item .

F2021L00339:89 a legcons:Item,
        owl:Class,
        dcat:Resource ;
    rdfs:label "Item - I89 11 3  Organic goods certificates"@en-AU ;
    dct:isPartOf F2021L00339:86 ;
    dct:isReferencedBy F2021L00339: ;
    rdfs:comment "11 3  Organic goods certificates - Abrievated Graph Key: I89"@en-AU ;
    skos:definition "11 3  Organic goods certificates"@en-AU ;
    skos:narrower F2021L00339:86 ;
    skos:prefLabel "Item I89"@en-AU ;
    dcat:accessURL <https://www.legislation.gov.au/F2021L00339/2023-08-04/2023-08-04/text/original/epub/OEBPS/document_1/document_1.html#_Toc143615226> ;
    dcat:landingPage "https://www.legislation.gov.au/F2021L00339/2023-08-04/2023-08-04/text/original/epub/OEBPS/document_1/document_1.html#_Toc143615226"^^xsd:anyURI ;
    dcat:theme legcons:Item .

F2021L00339:90 a legcons:Item,
        owl:Class,
        dcat:Resource ;
    rdfs:label "Item - I90 11 4  Records to be retained by exporter"@en-AU ;
    dct:isPartOf F2021L00339:86 ;
    dct:isReferencedBy F2021L00339: ;
    rdfs:comment "11 4  Records to be retained by exporter - Abrievated Graph Key: I90"@en-AU ;
    skos:definition "11 4  Records to be retained by exporter"@en-AU ;
    skos:narrower F2021L00339:86 ;
    skos:prefLabel "Item I90"@en-AU ;
    dcat:accessURL <https://www.legislation.gov.au/F2021L00339/2023-08-04/2023-08-04/text/original/epub/OEBPS/document_1/document_1.html#_Toc143615227> ;
    dcat:landingPage "https://www.legislation.gov.au/F2021L00339/2023-08-04/2023-08-04/text/original/epub/OEBPS/document_1/document_1.html#_Toc143615227"^^xsd:anyURI ;
    dcat:theme legcons:Item .

F2021L00339:91 a legcons:Item,
        owl:Class,
        dcat:Resource ;
    rdfs:label "Item - I91 11 5  Records to be retained by organic operator"@en-AU ;
    dct:isPartOf F2021L00339:86 ;
    dct:isReferencedBy F2021L00339: ;
    rdfs:comment "11 5  Records to be retained by organic operator - Abrievated Graph Key: I91"@en-AU ;
    skos:definition "11 5  Records to be retained by organic operator"@en-AU ;
    skos:narrower F2021L00339:86 ;
    skos:prefLabel "Item I91"@en-AU ;
    dcat:accessURL <https://www.legislation.gov.au/F2021L00339/2023-08-04/2023-08-04/text/original/epub/OEBPS/document_1/document_1.html#_Toc143615228> ;
    dcat:landingPage "https://www.legislation.gov.au/F2021L00339/2023-08-04/2023-08-04/text/original/epub/OEBPS/document_1/document_1.html#_Toc143615228"^^xsd:anyURI ;
    dcat:theme legcons:Item .

F2021L00339:92 a legcons:Item,
        owl:Class,
        dcat:Resource ;
    rdfs:label "Item - I92 11 6  Records to be retained by holder of approved arrangement"@en-AU ;
    dct:isPartOf F2021L00339:86 ;
    dct:isReferencedBy F2021L00339: ;
    rdfs:comment "11 6  Records to be retained by holder of approved arrangement - Abrievated Graph Key: I92"@en-AU ;
    skos:definition "11 6  Records to be retained by holder of approved arrangement"@en-AU ;
    skos:narrower F2021L00339:86 ;
    skos:prefLabel "Item I92"@en-AU ;
    dcat:accessURL <https://www.legislation.gov.au/F2021L00339/2023-08-04/2023-08-04/text/original/epub/OEBPS/document_1/document_1.html#_Toc143615229> ;
    dcat:landingPage "https://www.legislation.gov.au/F2021L00339/2023-08-04/2023-08-04/text/original/epub/OEBPS/document_1/document_1.html#_Toc143615229"^^xsd:anyURI ;
    dcat:theme legcons:Item .

F2021L00339:93 a legcons:Item,
        owl:Class,
        dcat:Resource ;
    rdfs:label "Item - I93 11 7  Records must not be altered or defaced during retention period"@en-AU ;
    dct:isPartOf F2021L00339:86 ;
    dct:isReferencedBy F2021L00339: ;
    rdfs:comment "11 7  Records must not be altered or defaced during retention period - Abrievated Graph Key: I93"@en-AU ;
    skos:definition "11 7  Records must not be altered or defaced during retention period"@en-AU ;
    skos:narrower F2021L00339:86 ;
    skos:prefLabel "Item I93"@en-AU ;
    dcat:accessURL <https://www.legislation.gov.au/F2021L00339/2023-08-04/2023-08-04/text/original/epub/OEBPS/document_1/document_1.html#_Toc143615230> ;
    dcat:landingPage "https://www.legislation.gov.au/F2021L00339/2023-08-04/2023-08-04/text/original/epub/OEBPS/document_1/document_1.html#_Toc143615230"^^xsd:anyURI ;
    dcat:theme legcons:Item .

F2021L00339:95 a legcons:Item,
        owl:Class,
        dcat:Resource ;
    rdfs:label "Item - I95 11 8  Storage of samples"@en-AU ;
    dct:isPartOf F2021L00339:94 ;
    dct:isReferencedBy F2021L00339: ;
    rdfs:comment "11 8  Storage of samples - Abrievated Graph Key: I95"@en-AU ;
    skos:definition "11 8  Storage of samples"@en-AU ;
    skos:narrower F2021L00339:94 ;
    skos:prefLabel "Item I95"@en-AU ;
    dcat:accessURL <https://www.legislation.gov.au/F2021L00339/2023-08-04/2023-08-04/text/original/epub/OEBPS/document_1/document_1.html#_Toc143615232> ;
    dcat:landingPage "https://www.legislation.gov.au/F2021L00339/2023-08-04/2023-08-04/text/original/epub/OEBPS/document_1/document_1.html#_Toc143615232"^^xsd:anyURI ;
    dcat:theme legcons:Item .

F2021L00339:97 a legcons:Item,
        owl:Class,
        dcat:Resource ;
    rdfs:label "Item - I97 11 9  Division of compensation between owners"@en-AU ;
    dct:isPartOf F2021L00339:96 ;
    dct:isReferencedBy F2021L00339: ;
    rdfs:comment "11 9  Division of compensation between owners - Abrievated Graph Key: I97"@en-AU ;
    skos:definition "11 9  Division of compensation between owners"@en-AU ;
    skos:narrower F2021L00339:96 ;
    skos:prefLabel "Item I97"@en-AU ;
    dcat:accessURL <https://www.legislation.gov.au/F2021L00339/2023-08-04/2023-08-04/text/original/epub/OEBPS/document_1/document_1.html#_Toc143615234> ;
    dcat:landingPage "https://www.legislation.gov.au/F2021L00339/2023-08-04/2023-08-04/text/original/epub/OEBPS/document_1/document_1.html#_Toc143615234"^^xsd:anyURI ;
    dcat:theme legcons:Item .

F2021L00339:98 a legcons:Item,
        owl:Class,
        dcat:Resource ;
    rdfs:label "Item - I98 11 10  Amount of compensation"@en-AU ;
    dct:isPartOf F2021L00339:96 ;
    dct:isReferencedBy F2021L00339: ;
    rdfs:comment "11 10  Amount of compensation - Abrievated Graph Key: I98"@en-AU ;
    skos:definition "11 10  Amount of compensation"@en-AU ;
    skos:narrower F2021L00339:96 ;
    skos:prefLabel "Item I98"@en-AU ;
    dcat:accessURL <https://www.legislation.gov.au/F2021L00339/2023-08-04/2023-08-04/text/original/epub/OEBPS/document_1/document_1.html#_Toc143615235> ;
    dcat:landingPage "https://www.legislation.gov.au/F2021L00339/2023-08-04/2023-08-04/text/original/epub/OEBPS/document_1/document_1.html#_Toc143615235"^^xsd:anyURI ;
    dcat:theme legcons:Item .

F2021L00339:102 a legcons:Part,
        owl:Class,
        dcat:Resource ;
    rdfs:label "Part - P102 Part 1 Preliminary"@en-AU ;
    dct:hasPart F2021L00339:103 ;
    dct:isPartOf F2021L00339:101 ;
    dct:isReferencedBy F2021L00339: ;
    rdfs:comment "Part 1 Preliminary - Abrievated Graph Key: P102"@en-AU ;
    skos:broader F2021L00339:103 ;
    skos:definition "Part 1 Preliminary"@en-AU ;
    skos:narrower F2021L00339:101 ;
    skos:prefLabel "Part P102"@en-AU ;
    dcat:accessURL <https://www.legislation.gov.au/F2021L00339/2023-08-04/2023-08-04/text/original/epub/OEBPS/document_1/document_1.html#_Toc143615239> ;
    dcat:landingPage "https://www.legislation.gov.au/F2021L00339/2023-08-04/2023-08-04/text/original/epub/OEBPS/document_1/document_1.html#_Toc143615239"^^xsd:anyURI ;
    dcat:theme legcons:Part .

F2021L00339:35 a legcons:Part,
        owl:Class,
        dcat:Resource ;
    rdfs:label "Part - P35 Part 1 Requirements for approval"@en-AU ;
    dct:hasPart F2021L00339:36 ;
    dct:isPartOf F2021L00339:34 ;
    dct:isReferencedBy F2021L00339: ;
    rdfs:comment "Part 1 Requirements for approval - Abrievated Graph Key: P35"@en-AU ;
    skos:broader F2021L00339:36 ;
    skos:definition "Part 1 Requirements for approval"@en-AU ;
    skos:narrower F2021L00339:34 ;
    skos:prefLabel "Part P35"@en-AU ;
    dcat:accessURL <https://www.legislation.gov.au/F2021L00339/2023-08-04/2023-08-04/text/original/epub/OEBPS/document_1/document_1.html#_Toc143615172> ;
    dcat:landingPage "https://www.legislation.gov.au/F2021L00339/2023-08-04/2023-08-04/text/original/epub/OEBPS/document_1/document_1.html#_Toc143615172"^^xsd:anyURI ;
    dcat:theme legcons:Part .

F2021L00339:38 a legcons:Division,
        owl:Class,
        dcat:Resource ;
    rdfs:label "Division - D38 Division 1 Purpose of this Part"@en-AU ;
    dct:hasPart F2021L00339:39 ;
    dct:isPartOf F2021L00339:37 ;
    dct:isReferencedBy F2021L00339: ;
    rdfs:comment "Division 1 Purpose of this Part - Abrievated Graph Key: D38"@en-AU ;
    skos:broader F2021L00339:39 ;
    skos:definition "Division 1 Purpose of this Part"@en-AU ;
    skos:narrower F2021L00339:37 ;
    skos:prefLabel "Division D38"@en-AU ;
    dcat:accessURL <https://www.legislation.gov.au/F2021L00339/2023-08-04/2023-08-04/text/original/epub/OEBPS/document_1/document_1.html#_Toc143615175> ;
    dcat:landingPage "https://www.legislation.gov.au/F2021L00339/2023-08-04/2023-08-04/text/original/epub/OEBPS/document_1/document_1.html#_Toc143615175"^^xsd:anyURI ;
    dcat:theme legcons:Division .

F2021L00339:51 a legcons:Part,
        owl:Class,
        dcat:Resource ;
    rdfs:label "Part - P51 Part 3 Renewal of approved arrangement"@en-AU ;
    dct:hasPart F2021L00339:52 ;
    dct:isPartOf F2021L00339:34 ;
    dct:isReferencedBy F2021L00339: ;
    rdfs:comment "Part 3 Renewal of approved arrangement - Abrievated Graph Key: P51"@en-AU ;
    skos:broader F2021L00339:52 ;
    skos:definition "Part 3 Renewal of approved arrangement"@en-AU ;
    skos:narrower F2021L00339:34 ;
    skos:prefLabel "Part P51"@en-AU ;
    dcat:accessURL <https://www.legislation.gov.au/F2021L00339/2023-08-04/2023-08-04/text/original/epub/OEBPS/document_1/document_1.html#_Toc143615188> ;
    dcat:landingPage "https://www.legislation.gov.au/F2021L00339/2023-08-04/2023-08-04/text/original/epub/OEBPS/document_1/document_1.html#_Toc143615188"^^xsd:anyURI ;
    dcat:theme legcons:Part .

F2021L00339:54 a legcons:Division,
        owl:Class,
        dcat:Resource ;
    rdfs:label "Division - D54 Division 1 Variations by holder"@en-AU ;
    dct:hasPart F2021L00339:55 ;
    dct:isPartOf F2021L00339:53 ;
    dct:isReferencedBy F2021L00339: ;
    rdfs:comment "Division 1 Variations by holder - Abrievated Graph Key: D54"@en-AU ;
    skos:broader F2021L00339:55 ;
    skos:definition "Division 1 Variations by holder"@en-AU ;
    skos:narrower F2021L00339:53 ;
    skos:prefLabel "Division D54"@en-AU ;
    dcat:accessURL <https://www.legislation.gov.au/F2021L00339/2023-08-04/2023-08-04/text/original/epub/OEBPS/document_1/document_1.html#_Toc143615191> ;
    dcat:landingPage "https://www.legislation.gov.au/F2021L00339/2023-08-04/2023-08-04/text/original/epub/OEBPS/document_1/document_1.html#_Toc143615191"^^xsd:anyURI ;
    dcat:theme legcons:Division .

F2021L00339:56 a legcons:Division,
        owl:Class,
        dcat:Resource ;
    rdfs:label "Division - D56 Division 2 Variations required by Secretary"@en-AU ;
    dct:hasPart F2021L00339:57 ;
    dct:isPartOf F2021L00339:53 ;
    dct:isReferencedBy F2021L00339: ;
    rdfs:comment "Division 2 Variations required by Secretary - Abrievated Graph Key: D56"@en-AU ;
    skos:broader F2021L00339:57 ;
    skos:definition "Division 2 Variations required by Secretary"@en-AU ;
    skos:narrower F2021L00339:53 ;
    skos:prefLabel "Division D56"@en-AU ;
    dcat:accessURL <https://www.legislation.gov.au/F2021L00339/2023-08-04/2023-08-04/text/original/epub/OEBPS/document_1/document_1.html#_Toc143615193> ;
    dcat:landingPage "https://www.legislation.gov.au/F2021L00339/2023-08-04/2023-08-04/text/original/epub/OEBPS/document_1/document_1.html#_Toc143615193"^^xsd:anyURI ;
    dcat:theme legcons:Division .

F2021L00339:58 a legcons:Part,
        owl:Class,
        dcat:Resource ;
    rdfs:label "Part - P58 Part 5 Obligations of holders of approved arrangements etc"@en-AU ;
    dct:hasPart F2021L00339:59 ;
    dct:isPartOf F2021L00339:34 ;
    dct:isReferencedBy F2021L00339: ;
    rdfs:comment "Part 5 Obligations of holders of approved arrangements etc - Abrievated Graph Key: P58"@en-AU ;
    skos:broader F2021L00339:59 ;
    skos:definition "Part 5 Obligations of holders of approved arrangements etc"@en-AU ;
    skos:narrower F2021L00339:34 ;
    skos:prefLabel "Part P58"@en-AU ;
    dcat:accessURL <https://www.legislation.gov.au/F2021L00339/2023-08-04/2023-08-04/text/original/epub/OEBPS/document_1/document_1.html#_Toc143615195> ;
    dcat:landingPage "https://www.legislation.gov.au/F2021L00339/2023-08-04/2023-08-04/text/original/epub/OEBPS/document_1/document_1.html#_Toc143615195"^^xsd:anyURI ;
    dcat:theme legcons:Part .

F2021L00339:60 a legcons:Part,
        owl:Class,
        dcat:Resource ;
    rdfs:label "Part - P60 Part 6 Fit and proper persons"@en-AU ;
    dct:hasPart F2021L00339:61 ;
    dct:isPartOf F2021L00339:34 ;
    dct:isReferencedBy F2021L00339: ;
    rdfs:comment "Part 6 Fit and proper persons - Abrievated Graph Key: P60"@en-AU ;
    skos:broader F2021L00339:61 ;
    skos:definition "Part 6 Fit and proper persons"@en-AU ;
    skos:narrower F2021L00339:34 ;
    skos:prefLabel "Part P60"@en-AU ;
    dcat:accessURL <https://www.legislation.gov.au/F2021L00339/2023-08-04/2023-08-04/text/original/epub/OEBPS/document_1/document_1.html#_Toc143615197> ;
    dcat:landingPage "https://www.legislation.gov.au/F2021L00339/2023-08-04/2023-08-04/text/original/epub/OEBPS/document_1/document_1.html#_Toc143615197"^^xsd:anyURI ;
    dcat:theme legcons:Part .

F2021L00339:72 a legcons:Chapter,
        owl:Class,
        dcat:Resource ;
    rdfs:label "Chapter - C72 Chapter 9 Powers and officials"@en-AU ;
    dct:hasPart F2021L00339:73,
        F2021L00339:80 ;
    dct:isReferencedBy F2021L00339: ;
    rdfs:comment "Chapter 9 Powers and officials - Abrievated Graph Key: C72"@en-AU ;
    skos:broader F2021L00339:73,
        F2021L00339:80 ;
    skos:definition "Chapter 9 Powers and officials"@en-AU ;
    skos:prefLabel "Chapter C72"@en-AU ;
    dcat:accessURL <https://www.legislation.gov.au/F2021L00339/2023-08-04/2023-08-04/text/original/epub/OEBPS/document_1/document_1.html#_Toc143615209> ;
    dcat:landingPage "https://www.legislation.gov.au/F2021L00339/2023-08-04/2023-08-04/text/original/epub/OEBPS/document_1/document_1.html#_Toc143615209"^^xsd:anyURI ;
    dcat:theme legcons:Chapter .

F2021L00339:74 a legcons:Division,
        owl:Class,
        dcat:Resource ;
    rdfs:label "Division - D74 Division 1 General"@en-AU ;
    dct:hasPart F2021L00339:75 ;
    dct:isPartOf F2021L00339:73 ;
    dct:isReferencedBy F2021L00339: ;
    rdfs:comment "Division 1 General - Abrievated Graph Key: D74"@en-AU ;
    skos:broader F2021L00339:75 ;
    skos:definition "Division 1 General"@en-AU ;
    skos:narrower F2021L00339:73 ;
    skos:prefLabel "Division D74"@en-AU ;
    dcat:accessURL <https://www.legislation.gov.au/F2021L00339/2023-08-04/2023-08-04/text/original/epub/OEBPS/document_1/document_1.html#_Toc143615211> ;
    dcat:landingPage "https://www.legislation.gov.au/F2021L00339/2023-08-04/2023-08-04/text/original/epub/OEBPS/document_1/document_1.html#_Toc143615211"^^xsd:anyURI ;
    dcat:theme legcons:Division .

F2021L00339:80 a legcons:Part,
        owl:Class,
        dcat:Resource ;
    rdfs:label "Part - P80 Part 2 Authorised officers"@en-AU ;
    dct:hasPart F2021L00339:81 ;
    dct:isPartOf F2021L00339:72 ;
    dct:isReferencedBy F2021L00339: ;
    rdfs:comment "Part 2 Authorised officers - Abrievated Graph Key: P80"@en-AU ;
    skos:broader F2021L00339:81 ;
    skos:definition "Part 2 Authorised officers"@en-AU ;
    skos:narrower F2021L00339:72 ;
    skos:prefLabel "Part P80"@en-AU ;
    dcat:accessURL <https://www.legislation.gov.au/F2021L00339/2023-08-04/2023-08-04/text/original/epub/OEBPS/document_1/document_1.html#_Toc143615217> ;
    dcat:landingPage "https://www.legislation.gov.au/F2021L00339/2023-08-04/2023-08-04/text/original/epub/OEBPS/document_1/document_1.html#_Toc143615217"^^xsd:anyURI ;
    dcat:theme legcons:Part .

F2021L00339:82 a legcons:Chapter,
        owl:Class,
        dcat:Resource ;
    rdfs:label "Chapter - C82 Chapter 10 Compliance and enforcement"@en-AU ;
    dct:hasPart F2021L00339:83,
        F2021L00339:84 ;
    dct:isReferencedBy F2021L00339: ;
    rdfs:comment "Chapter 10 Compliance and enforcement - Abrievated Graph Key: C82"@en-AU ;
    skos:broader F2021L00339:83,
        F2021L00339:84 ;
    skos:definition "Chapter 10 Compliance and enforcement"@en-AU ;
    skos:prefLabel "Chapter C82"@en-AU ;
    dcat:accessURL <https://www.legislation.gov.au/F2021L00339/2023-08-04/2023-08-04/text/original/epub/OEBPS/document_1/document_1.html#_Toc143615219> ;
    dcat:landingPage "https://www.legislation.gov.au/F2021L00339/2023-08-04/2023-08-04/text/original/epub/OEBPS/document_1/document_1.html#_Toc143615219"^^xsd:anyURI ;
    dcat:theme legcons:Chapter .

F2021L00339:94 a legcons:Part,
        owl:Class,
        dcat:Resource ;
    rdfs:label "Part - P94 Part 2 Samples"@en-AU ;
    dct:hasPart F2021L00339:95 ;
    dct:isPartOf F2021L00339:85 ;
    dct:isReferencedBy F2021L00339: ;
    rdfs:comment "Part 2 Samples - Abrievated Graph Key: P94"@en-AU ;
    skos:broader F2021L00339:95 ;
    skos:definition "Part 2 Samples"@en-AU ;
    skos:narrower F2021L00339:85 ;
    skos:prefLabel "Part P94"@en-AU ;
    dcat:accessURL <https://www.legislation.gov.au/F2021L00339/2023-08-04/2023-08-04/text/original/epub/OEBPS/document_1/document_1.html#_Toc143615231> ;
    dcat:landingPage "https://www.legislation.gov.au/F2021L00339/2023-08-04/2023-08-04/text/original/epub/OEBPS/document_1/document_1.html#_Toc143615231"^^xsd:anyURI ;
    dcat:theme legcons:Part .

F2021L00339:99 a legcons:Part,
        owl:Class,
        dcat:Resource ;
    rdfs:label "Part - P99 Part 4 Relevant Commonwealth liabilities"@en-AU ;
    dct:hasPart F2021L00339:100 ;
    dct:isPartOf F2021L00339:85 ;
    dct:isReferencedBy F2021L00339: ;
    rdfs:comment "Part 4 Relevant Commonwealth liabilities - Abrievated Graph Key: P99"@en-AU ;
    skos:broader F2021L00339:100 ;
    skos:definition "Part 4 Relevant Commonwealth liabilities"@en-AU ;
    skos:narrower F2021L00339:85 ;
    skos:prefLabel "Part P99"@en-AU ;
    dcat:accessURL <https://www.legislation.gov.au/F2021L00339/2023-08-04/2023-08-04/text/original/epub/OEBPS/document_1/document_1.html#_Toc143615236> ;
    dcat:landingPage "https://www.legislation.gov.au/F2021L00339/2023-08-04/2023-08-04/text/original/epub/OEBPS/document_1/document_1.html#_Toc143615236"^^xsd:anyURI ;
    dcat:theme legcons:Part .

F2021L00339:101 a legcons:Chapter,
        owl:Class,
        dcat:Resource ;
    rdfs:label "Chapter - C101 Chapter 12 Transitional provisions"@en-AU ;
    dct:hasPart F2021L00339:102,
        F2021L00339:104,
        F2021L00339:111 ;
    dct:isReferencedBy F2021L00339: ;
    rdfs:comment "Chapter 12 Transitional provisions - Abrievated Graph Key: C101"@en-AU ;
    skos:broader F2021L00339:102,
        F2021L00339:104,
        F2021L00339:111 ;
    skos:definition "Chapter 12 Transitional provisions"@en-AU ;
    skos:prefLabel "Chapter C101"@en-AU ;
    dcat:accessURL <https://www.legislation.gov.au/F2021L00339/2023-08-04/2023-08-04/text/original/epub/OEBPS/document_1/document_1.html#_Toc143615238> ;
    dcat:landingPage "https://www.legislation.gov.au/F2021L00339/2023-08-04/2023-08-04/text/original/epub/OEBPS/document_1/document_1.html#_Toc143615238"^^xsd:anyURI ;
    dcat:theme legcons:Chapter .

F2021L00339:11 a legcons:Division,
        owl:Class,
        dcat:Resource ;
    rdfs:label "Division - D11 Division 1 Prescribed goods"@en-AU ;
    dct:hasPart F2021L00339:12,
        F2021L00339:13 ;
    dct:isPartOf F2021L00339:10 ;
    dct:isReferencedBy F2021L00339: ;
    rdfs:comment "Division 1 Prescribed goods - Abrievated Graph Key: D11"@en-AU ;
    skos:broader F2021L00339:12,
        F2021L00339:13 ;
    skos:definition "Division 1 Prescribed goods"@en-AU ;
    skos:narrower F2021L00339:10 ;
    skos:prefLabel "Division D11"@en-AU ;
    dcat:accessURL <https://www.legislation.gov.au/F2021L00339/2023-08-04/2023-08-04/text/original/epub/OEBPS/document_1/document_1.html#_Toc143615148> ;
    dcat:landingPage "https://www.legislation.gov.au/F2021L00339/2023-08-04/2023-08-04/text/original/epub/OEBPS/document_1/document_1.html#_Toc143615148"^^xsd:anyURI ;
    dcat:theme legcons:Division .

F2021L00339:53 a legcons:Part,
        owl:Class,
        dcat:Resource ;
    rdfs:label "Part - P53 Part 4 Variation of approved arrangement"@en-AU ;
    dct:hasPart F2021L00339:54,
        F2021L00339:56 ;
    dct:isPartOf F2021L00339:34 ;
    dct:isReferencedBy F2021L00339: ;
    rdfs:comment "Part 4 Variation of approved arrangement - Abrievated Graph Key: P53"@en-AU ;
    skos:broader F2021L00339:54,
        F2021L00339:56 ;
    skos:definition "Part 4 Variation of approved arrangement"@en-AU ;
    skos:narrower F2021L00339:34 ;
    skos:prefLabel "Part P53"@en-AU ;
    dcat:accessURL <https://www.legislation.gov.au/F2021L00339/2023-08-04/2023-08-04/text/original/epub/OEBPS/document_1/document_1.html#_Toc143615190> ;
    dcat:landingPage "https://www.legislation.gov.au/F2021L00339/2023-08-04/2023-08-04/text/original/epub/OEBPS/document_1/document_1.html#_Toc143615190"^^xsd:anyURI ;
    dcat:theme legcons:Part .

F2021L00339:73 a legcons:Part,
        owl:Class,
        dcat:Resource ;
    rdfs:label "Part - P73 Part 1 Audits"@en-AU ;
    dct:hasPart F2021L00339:74,
        F2021L00339:76 ;
    dct:isPartOf F2021L00339:72 ;
    dct:isReferencedBy F2021L00339: ;
    rdfs:comment "Part 1 Audits - Abrievated Graph Key: P73"@en-AU ;
    skos:broader F2021L00339:74,
        F2021L00339:76 ;
    skos:definition "Part 1 Audits"@en-AU ;
    skos:narrower F2021L00339:72 ;
    skos:prefLabel "Part P73"@en-AU ;
    dcat:accessURL <https://www.legislation.gov.au/F2021L00339/2023-08-04/2023-08-04/text/original/epub/OEBPS/document_1/document_1.html#_Toc143615210> ;
    dcat:landingPage "https://www.legislation.gov.au/F2021L00339/2023-08-04/2023-08-04/text/original/epub/OEBPS/document_1/document_1.html#_Toc143615210"^^xsd:anyURI ;
    dcat:theme legcons:Part .

F2021L00339:96 a legcons:Part,
        owl:Class,
        dcat:Resource ;
    rdfs:label "Part - P96 Part 3 Damaged or destroyed prescribed organic goods"@en-AU ;
    dct:hasPart F2021L00339:97,
        F2021L00339:98 ;
    dct:isPartOf F2021L00339:85 ;
    dct:isReferencedBy F2021L00339: ;
    rdfs:comment "Part 3 Damaged or destroyed prescribed organic goods - Abrievated Graph Key: P96"@en-AU ;
    skos:broader F2021L00339:97,
        F2021L00339:98 ;
    skos:definition "Part 3 Damaged or destroyed prescribed organic goods"@en-AU ;
    skos:narrower F2021L00339:85 ;
    skos:prefLabel "Part P96"@en-AU ;
    dcat:accessURL <https://www.legislation.gov.au/F2021L00339/2023-08-04/2023-08-04/text/original/epub/OEBPS/document_1/document_1.html#_Toc143615233> ;
    dcat:landingPage "https://www.legislation.gov.au/F2021L00339/2023-08-04/2023-08-04/text/original/epub/OEBPS/document_1/document_1.html#_Toc143615233"^^xsd:anyURI ;
    dcat:theme legcons:Part .

F2021L00339:37 a legcons:Part,
        owl:Class,
        dcat:Resource ;
    rdfs:label "Part - P37 Part 2 Conditions of approved arrangement"@en-AU ;
    dct:hasPart F2021L00339:38,
        F2021L00339:40,
        F2021L00339:44 ;
    dct:isPartOf F2021L00339:34 ;
    dct:isReferencedBy F2021L00339: ;
    rdfs:comment "Part 2 Conditions of approved arrangement - Abrievated Graph Key: P37"@en-AU ;
    skos:broader F2021L00339:38,
        F2021L00339:40,
        F2021L00339:44 ;
    skos:definition "Part 2 Conditions of approved arrangement"@en-AU ;
    skos:narrower F2021L00339:34 ;
    skos:prefLabel "Part P37"@en-AU ;
    dcat:accessURL <https://www.legislation.gov.au/F2021L00339/2023-08-04/2023-08-04/text/original/epub/OEBPS/document_1/document_1.html#_Toc143615174> ;
    dcat:landingPage "https://www.legislation.gov.au/F2021L00339/2023-08-04/2023-08-04/text/original/epub/OEBPS/document_1/document_1.html#_Toc143615174"^^xsd:anyURI ;
    dcat:theme legcons:Part .

F2021L00339:40 a legcons:Division,
        owl:Class,
        dcat:Resource ;
    rdfs:label "Division - D40 Division 2 General"@en-AU ;
    dct:hasPart F2021L00339:41,
        F2021L00339:42,
        F2021L00339:43 ;
    dct:isPartOf F2021L00339:37 ;
    dct:isReferencedBy F2021L00339: ;
    rdfs:comment "Division 2 General - Abrievated Graph Key: D40"@en-AU ;
    skos:broader F2021L00339:41,
        F2021L00339:42,
        F2021L00339:43 ;
    skos:definition "Division 2 General"@en-AU ;
    skos:narrower F2021L00339:37 ;
    skos:prefLabel "Division D40"@en-AU ;
    dcat:accessURL <https://www.legislation.gov.au/F2021L00339/2023-08-04/2023-08-04/text/original/epub/OEBPS/document_1/document_1.html#_Toc143615177> ;
    dcat:landingPage "https://www.legislation.gov.au/F2021L00339/2023-08-04/2023-08-04/text/original/epub/OEBPS/document_1/document_1.html#_Toc143615177"^^xsd:anyURI ;
    dcat:theme legcons:Division .

F2021L00339:62 a legcons:Part,
        owl:Class,
        dcat:Resource ;
    rdfs:label "Part - P62 Part 7 Matters relating to applications"@en-AU ;
    dct:hasPart F2021L00339:63,
        F2021L00339:64,
        F2021L00339:65 ;
    dct:isPartOf F2021L00339:34 ;
    dct:isReferencedBy F2021L00339: ;
    rdfs:comment "Part 7 Matters relating to applications - Abrievated Graph Key: P62"@en-AU ;
    skos:broader F2021L00339:63,
        F2021L00339:64,
        F2021L00339:65 ;
    skos:definition "Part 7 Matters relating to applications"@en-AU ;
    skos:narrower F2021L00339:34 ;
    skos:prefLabel "Part P62"@en-AU ;
    dcat:accessURL <https://www.legislation.gov.au/F2021L00339/2023-08-04/2023-08-04/text/original/epub/OEBPS/document_1/document_1.html#_Toc143615199> ;
    dcat:landingPage "https://www.legislation.gov.au/F2021L00339/2023-08-04/2023-08-04/text/original/epub/OEBPS/document_1/document_1.html#_Toc143615199"^^xsd:anyURI ;
    dcat:theme legcons:Part .

F2021L00339:76 a legcons:Division,
        owl:Class,
        dcat:Resource ;
    rdfs:label "Division - D76 Division 2 Conduct of audit etc"@en-AU ;
    dct:hasPart F2021L00339:77,
        F2021L00339:78,
        F2021L00339:79 ;
    dct:isPartOf F2021L00339:73 ;
    dct:isReferencedBy F2021L00339: ;
    rdfs:comment "Division 2 Conduct of audit etc - Abrievated Graph Key: D76"@en-AU ;
    skos:broader F2021L00339:77,
        F2021L00339:78,
        F2021L00339:79 ;
    skos:definition "Division 2 Conduct of audit etc"@en-AU ;
    skos:narrower F2021L00339:73 ;
    skos:prefLabel "Division D76"@en-AU ;
    dcat:accessURL <https://www.legislation.gov.au/F2021L00339/2023-08-04/2023-08-04/text/original/epub/OEBPS/document_1/document_1.html#_Toc143615213> ;
    dcat:landingPage "https://www.legislation.gov.au/F2021L00339/2023-08-04/2023-08-04/text/original/epub/OEBPS/document_1/document_1.html#_Toc143615213"^^xsd:anyURI ;
    dcat:theme legcons:Division .

F2021L00339:85 a legcons:Chapter,
        owl:Class,
        dcat:Resource ;
    rdfs:label "Chapter - C85 Chapter 11 Miscellaneous"@en-AU ;
    dct:hasPart F2021L00339:86,
        F2021L00339:94,
        F2021L00339:96,
        F2021L00339:99 ;
    dct:isReferencedBy F2021L00339: ;
    rdfs:comment "Chapter 11 Miscellaneous - Abrievated Graph Key: C85"@en-AU ;
    skos:broader F2021L00339:86,
        F2021L00339:94,
        F2021L00339:96,
        F2021L00339:99 ;
    skos:definition "Chapter 11 Miscellaneous"@en-AU ;
    skos:prefLabel "Chapter C85"@en-AU ;
    dcat:accessURL <https://www.legislation.gov.au/F2021L00339/2023-08-04/2023-08-04/text/original/epub/OEBPS/document_1/document_1.html#_Toc143615222> ;
    dcat:landingPage "https://www.legislation.gov.au/F2021L00339/2023-08-04/2023-08-04/text/original/epub/OEBPS/document_1/document_1.html#_Toc143615222"^^xsd:anyURI ;
    dcat:theme legcons:Chapter .

F2021L00339:10 a legcons:Part,
        owl:Class,
        dcat:Resource ;
    rdfs:label "Part - P10 Part 1 Goods"@en-AU ;
    dct:hasPart F2021L00339:11,
        F2021L00339:14,
        F2021L00339:15,
        F2021L00339:16 ;
    dct:isPartOf F2021L00339:9 ;
    dct:isReferencedBy F2021L00339: ;
    rdfs:comment "Part 1 Goods - Abrievated Graph Key: P10"@en-AU ;
    skos:broader F2021L00339:11,
        F2021L00339:14,
        F2021L00339:15,
        F2021L00339:16 ;
    skos:definition "Part 1 Goods"@en-AU ;
    skos:narrower F2021L00339:9 ;
    skos:prefLabel "Part P10"@en-AU ;
    dcat:accessURL <https://www.legislation.gov.au/F2021L00339/2023-08-04/2023-08-04/text/original/epub/OEBPS/document_1/document_1.html#_Toc143615147> ;
    dcat:landingPage "https://www.legislation.gov.au/F2021L00339/2023-08-04/2023-08-04/text/original/epub/OEBPS/document_1/document_1.html#_Toc143615147"^^xsd:anyURI ;
    dcat:theme legcons:Part .

F2021L00339:111 a legcons:Endnotes,
        owl:Class,
        dcat:Resource ;
    rdfs:label "Endnotes - E111 Endnotes"@en-AU ;
    dct:hasPart F2021L00339:112,
        F2021L00339:113,
        F2021L00339:114,
        F2021L00339:115 ;
    dct:isPartOf F2021L00339:101 ;
    dct:isReferencedBy F2021L00339: ;
    rdfs:comment "Endnotes - Abrievated Graph Key: E111"@en-AU ;
    skos:broader F2021L00339:112,
        F2021L00339:113,
        F2021L00339:114,
        F2021L00339:115 ;
    skos:definition "Endnotes"@en-AU ;
    skos:narrower F2021L00339:101 ;
    skos:prefLabel "Endnotes E111"@en-AU ;
    dcat:accessURL <https://www.legislation.gov.au/F2021L00339/2023-08-04/2023-08-04/text/original/epub/OEBPS/document_1/document_1.html#_Toc143615248> ;
    dcat:landingPage "https://www.legislation.gov.au/F2021L00339/2023-08-04/2023-08-04/text/original/epub/OEBPS/document_1/document_1.html#_Toc143615248"^^xsd:anyURI ;
    dcat:theme legcons:Endnotes .

F2021L00339:67 a legcons:Part,
        owl:Class,
        dcat:Resource ;
    rdfs:label "Part - P67 Part 1 Trade descriptions"@en-AU ;
    dct:hasPart F2021L00339:68,
        F2021L00339:69,
        F2021L00339:70,
        F2021L00339:71 ;
    dct:isPartOf F2021L00339:66 ;
    dct:isReferencedBy F2021L00339: ;
    rdfs:comment "Part 1 Trade descriptions - Abrievated Graph Key: P67"@en-AU ;
    skos:broader F2021L00339:68,
        F2021L00339:69,
        F2021L00339:70,
        F2021L00339:71 ;
    skos:definition "Part 1 Trade descriptions"@en-AU ;
    skos:narrower F2021L00339:66 ;
    skos:prefLabel "Part P67"@en-AU ;
    dcat:accessURL <https://www.legislation.gov.au/F2021L00339/2023-08-04/2023-08-04/text/original/epub/OEBPS/document_1/document_1.html#_Toc143615204> ;
    dcat:landingPage "https://www.legislation.gov.au/F2021L00339/2023-08-04/2023-08-04/text/original/epub/OEBPS/document_1/document_1.html#_Toc143615204"^^xsd:anyURI ;
    dcat:theme legcons:Part .

F2021L00339:1 a legcons:Chapter,
        owl:Class,
        dcat:Resource ;
    rdfs:label "Chapter - C1 Chapter 1 Preliminary"@en-AU ;
    dct:hasPart F2021L00339:2,
        F2021L00339:3,
        F2021L00339:4,
        F2021L00339:5,
        F2021L00339:6,
        F2021L00339:7,
        F2021L00339:8 ;
    dct:isReferencedBy F2021L00339: ;
    rdfs:comment "Chapter 1 Preliminary - Abrievated Graph Key: C1"@en-AU ;
    skos:broader F2021L00339:2,
        F2021L00339:3,
        F2021L00339:4,
        F2021L00339:5,
        F2021L00339:6,
        F2021L00339:7,
        F2021L00339:8 ;
    skos:definition "Chapter 1 Preliminary"@en-AU ;
    skos:prefLabel "Chapter C1"@en-AU ;
    dcat:accessURL <https://www.legislation.gov.au/F2021L00339/2023-08-04/2023-08-04/text/original/epub/OEBPS/document_1/document_1.html#_Toc143615138> ;
    dcat:landingPage "https://www.legislation.gov.au/F2021L00339/2023-08-04/2023-08-04/text/original/epub/OEBPS/document_1/document_1.html#_Toc143615138"^^xsd:anyURI ;
    dcat:theme legcons:Chapter .

F2021L00339:104 a legcons:Part,
        owl:Class,
        dcat:Resource ;
    rdfs:label "Part - P104 Part 2 Approved arrangements"@en-AU ;
    dct:hasPart F2021L00339:105,
        F2021L00339:106,
        F2021L00339:107,
        F2021L00339:108,
        F2021L00339:109,
        F2021L00339:110 ;
    dct:isPartOf F2021L00339:101 ;
    dct:isReferencedBy F2021L00339: ;
    rdfs:comment "Part 2 Approved arrangements - Abrievated Graph Key: P104"@en-AU ;
    skos:broader F2021L00339:105,
        F2021L00339:106,
        F2021L00339:107,
        F2021L00339:108,
        F2021L00339:109,
        F2021L00339:110 ;
    skos:definition "Part 2 Approved arrangements"@en-AU ;
    skos:narrower F2021L00339:101 ;
    skos:prefLabel "Part P104"@en-AU ;
    dcat:accessURL <https://www.legislation.gov.au/F2021L00339/2023-08-04/2023-08-04/text/original/epub/OEBPS/document_1/document_1.html#_Toc143615241> ;
    dcat:landingPage "https://www.legislation.gov.au/F2021L00339/2023-08-04/2023-08-04/text/original/epub/OEBPS/document_1/document_1.html#_Toc143615241"^^xsd:anyURI ;
    dcat:theme legcons:Part .

F2021L00339:34 a legcons:Chapter,
        owl:Class,
        dcat:Resource ;
    rdfs:label "Chapter - C34 Chapter 5 Approved arrangements"@en-AU ;
    dct:hasPart F2021L00339:35,
        F2021L00339:37,
        F2021L00339:51,
        F2021L00339:53,
        F2021L00339:58,
        F2021L00339:60,
        F2021L00339:62 ;
    dct:isReferencedBy F2021L00339: ;
    rdfs:comment "Chapter 5 Approved arrangements - Abrievated Graph Key: C34"@en-AU ;
    skos:broader F2021L00339:35,
        F2021L00339:37,
        F2021L00339:51,
        F2021L00339:53,
        F2021L00339:58,
        F2021L00339:60,
        F2021L00339:62 ;
    skos:definition "Chapter 5 Approved arrangements"@en-AU ;
    skos:prefLabel "Chapter C34"@en-AU ;
    dcat:accessURL <https://www.legislation.gov.au/F2021L00339/2023-08-04/2023-08-04/text/original/epub/OEBPS/document_1/document_1.html#_Toc143615171> ;
    dcat:landingPage "https://www.legislation.gov.au/F2021L00339/2023-08-04/2023-08-04/text/original/epub/OEBPS/document_1/document_1.html#_Toc143615171"^^xsd:anyURI ;
    dcat:theme legcons:Chapter .

F2021L00339:44 a legcons:Division,
        owl:Class,
        dcat:Resource ;
    rdfs:label "Division - D44 Division 3 Management practices"@en-AU ;
    dct:hasPart F2021L00339:45,
        F2021L00339:46,
        F2021L00339:47,
        F2021L00339:48,
        F2021L00339:49,
        F2021L00339:50 ;
    dct:isPartOf F2021L00339:37 ;
    dct:isReferencedBy F2021L00339: ;
    rdfs:comment "Division 3 Management practices - Abrievated Graph Key: D44"@en-AU ;
    skos:broader F2021L00339:45,
        F2021L00339:46,
        F2021L00339:47,
        F2021L00339:48,
        F2021L00339:49,
        F2021L00339:50 ;
    skos:definition "Division 3 Management practices"@en-AU ;
    skos:narrower F2021L00339:37 ;
    skos:prefLabel "Division D44"@en-AU ;
    dcat:accessURL <https://www.legislation.gov.au/F2021L00339/2023-08-04/2023-08-04/text/original/epub/OEBPS/document_1/document_1.html#_Toc143615181> ;
    dcat:landingPage "https://www.legislation.gov.au/F2021L00339/2023-08-04/2023-08-04/text/original/epub/OEBPS/document_1/document_1.html#_Toc143615181"^^xsd:anyURI ;
    dcat:theme legcons:Division .

F2021L00339:86 a legcons:Part,
        owl:Class,
        dcat:Resource ;
    rdfs:label "Part - P86 Part 1 Records"@en-AU ;
    dct:hasPart F2021L00339:87,
        F2021L00339:88,
        F2021L00339:89,
        F2021L00339:90,
        F2021L00339:91,
        F2021L00339:92,
        F2021L00339:93 ;
    dct:isPartOf F2021L00339:85 ;
    dct:isReferencedBy F2021L00339: ;
    rdfs:comment "Part 1 Records - Abrievated Graph Key: P86"@en-AU ;
    skos:broader F2021L00339:87,
        F2021L00339:88,
        F2021L00339:89,
        F2021L00339:90,
        F2021L00339:91,
        F2021L00339:92,
        F2021L00339:93 ;
    skos:definition "Part 1 Records"@en-AU ;
    skos:narrower F2021L00339:85 ;
    skos:prefLabel "Part P86"@en-AU ;
    dcat:accessURL <https://www.legislation.gov.au/F2021L00339/2023-08-04/2023-08-04/text/original/epub/OEBPS/document_1/document_1.html#_Toc143615223> ;
    dcat:landingPage "https://www.legislation.gov.au/F2021L00339/2023-08-04/2023-08-04/text/original/epub/OEBPS/document_1/document_1.html#_Toc143615223"^^xsd:anyURI ;
    dcat:theme legcons:Part .

F2021L00339:9 a legcons:Chapter,
        owl:Class,
        dcat:Resource ;
    rdfs:label "Chapter - C9 Chapter 2 Exporting goods"@en-AU ;
    dct:hasPart F2021L00339:10,
        F2021L00339:17,
        F2021L00339:18,
        F2021L00339:19,
        F2021L00339:20,
        F2021L00339:21,
        F2021L00339:22,
        F2021L00339:23,
        F2021L00339:24,
        F2021L00339:25,
        F2021L00339:26,
        F2021L00339:27,
        F2021L00339:28,
        F2021L00339:29,
        F2021L00339:30,
        F2021L00339:31,
        F2021L00339:32,
        F2021L00339:33 ;
    dct:isReferencedBy F2021L00339: ;
    rdfs:comment "Chapter 2 Exporting goods - Abrievated Graph Key: C9"@en-AU ;
    skos:broader F2021L00339:10,
        F2021L00339:17,
        F2021L00339:18,
        F2021L00339:19,
        F2021L00339:20,
        F2021L00339:21,
        F2021L00339:22,
        F2021L00339:23,
        F2021L00339:24,
        F2021L00339:25,
        F2021L00339:26,
        F2021L00339:27,
        F2021L00339:28,
        F2021L00339:29,
        F2021L00339:30,
        F2021L00339:31,
        F2021L00339:32,
        F2021L00339:33 ;
    skos:definition "Chapter 2 Exporting goods"@en-AU ;
    skos:prefLabel "Chapter C9"@en-AU ;
    dcat:accessURL <https://www.legislation.gov.au/F2021L00339/2023-08-04/2023-08-04/text/original/epub/OEBPS/document_1/document_1.html#_Toc143615146> ;
    dcat:landingPage "https://www.legislation.gov.au/F2021L00339/2023-08-04/2023-08-04/text/original/epub/OEBPS/document_1/document_1.html#_Toc143615146"^^xsd:anyURI ;
    dcat:theme legcons:Chapter .

F2021L00339: a owl:Class,
        dcat:Dataset,
        dcat:Resource ;
    rdfs:label "Export Control (Organic Goods) Rules 2021" ;
    dct:Jurisdiction " Department of Agriculture, Fisheries and Forestry "@en-AU ;
    dct:created "2024-08-30T15:12:04.339293"^^xsd:dateTime ;
    dct:creator "https://orcid.org/0009-0007-8434-7325"^^xsd:anyURI ;
    dct:date "2023-08-04T00:00:00+10:00"^^xsd:dateTime ;
    dct:description "Export Control (Organic Goods) Rules 2021"@en-AU ;
    dct:identifier "https://www.legislation.gov.au/F2021L00339/latest"^^xsd:anyURI ;
    dct:license <https://creativecommons.org/licenses/by-sa/4.0/> ;
    dct:source "scheme=AGLSTERMS.AglsAgent; corporateName=Office Parliamentary Counsel; address=Locked Bag 30 Kingston ACT 2604; contact=+61 2 6120 1400"@en-AU ;
    dct:subject "Export Control (Organic Goods) Rules 2021"@en-AU ;
    dct:title "Export Control (Organic Goods) Rules 2021"@en-AU ;
    owl:imports legcons: ;
    dcat:theme legcons:Chapter,
        legcons:Division,
        legcons:Endnotes,
        legcons:Item,
        legcons:Part ;
    schema:identifier "F2021L00339" ;
    schema:status "In force" ;
    schema:version "F2023C00745 (C02)" .

