@prefix F2021L00310: <http://example.org/au/leg/dataset/F2021L00310/> .
@prefix dcat: <http://www.w3.org/ns/dcat#> .
@prefix dct: <http://purl.org/dc/terms/> .
@prefix legcons: <http://example.org/au/leg/concepts/> .
@prefix owl: <http://www.w3.org/2002/07/owl#> .
@prefix rdfs: <http://www.w3.org/2000/01/rdf-schema#> .
@prefix schema: <https://schema.org/> .
@prefix skos: <http://www.w3.org/2004/02/skos/core#> .
@prefix xsd: <http://www.w3.org/2001/XMLSchema#> .

F2021L00310:10 a legcons:Division,
        owl:Class,
        dcat:Resource ;
    rdfs:label "Division - D10 Division 2 Other interpretation provisions"@en-AU ;
    dct:isPartOf F2021L00310:1 ;
    dct:isReferencedBy F2021L00310: ;
    rdfs:comment "Division 2 Other interpretation provisions - Abrievated Graph Key: D10"@en-AU ;
    skos:definition "Division 2 Other interpretation provisions"@en-AU ;
    skos:narrower F2021L00310:1 ;
    skos:prefLabel "Division D10"@en-AU ;
    dcat:accessURL <https://www.legislation.gov.au/F2021L00310/2023-08-04/2023-08-04/text/1/epub/OEBPS/document_1/document_1.html#_Toc145601336> ;
    dcat:landingPage "https://www.legislation.gov.au/F2021L00310/2023-08-04/2023-08-04/text/1/epub/OEBPS/document_1/document_1.html#_Toc145601336"^^xsd:anyURI ;
    dcat:theme legcons:Division .

F2021L00310:100 a legcons:Item,
        owl:Class,
        dcat:Resource ;
    rdfs:label "Item - I100 5 18  Trade description must be applied to prescribed poultry meat and poultry meat products that are intended to be exported"@en-AU ;
    dct:isPartOf F2021L00310:99 ;
    dct:isReferencedBy F2021L00310: ;
    rdfs:comment "5 18  Trade description must be applied to prescribed poultry meat and poultry meat products that are intended to be exported - Abrievated Graph Key: I100"@en-AU ;
    skos:definition "5 18  Trade description must be applied to prescribed poultry meat and poultry meat products that are intended to be exported"@en-AU ;
    skos:narrower F2021L00310:99 ;
    skos:prefLabel "Item I100"@en-AU ;
    dcat:accessURL <https://www.legislation.gov.au/F2021L00310/2023-08-04/2023-08-04/text/1/epub/OEBPS/document_1/document_1.html#_Toc145601426> ;
    dcat:landingPage "https://www.legislation.gov.au/F2021L00310/2023-08-04/2023-08-04/text/1/epub/OEBPS/document_1/document_1.html#_Toc145601426"^^xsd:anyURI ;
    dcat:theme legcons:Item .

F2021L00310:101 a legcons:Item,
        owl:Class,
        dcat:Resource ;
    rdfs:label "Item - I101 5 19  Prescribed poultry meat or poultry meat products in cartons or cans"@en-AU ;
    dct:isPartOf F2021L00310:99 ;
    dct:isReferencedBy F2021L00310: ;
    rdfs:comment "5 19  Prescribed poultry meat or poultry meat products in cartons or cans - Abrievated Graph Key: I101"@en-AU ;
    skos:definition "5 19  Prescribed poultry meat or poultry meat products in cartons or cans"@en-AU ;
    skos:narrower F2021L00310:99 ;
    skos:prefLabel "Item I101"@en-AU ;
    dcat:accessURL <https://www.legislation.gov.au/F2021L00310/2023-08-04/2023-08-04/text/1/epub/OEBPS/document_1/document_1.html#_Toc145601427> ;
    dcat:landingPage "https://www.legislation.gov.au/F2021L00310/2023-08-04/2023-08-04/text/1/epub/OEBPS/document_1/document_1.html#_Toc145601427"^^xsd:anyURI ;
    dcat:theme legcons:Item .

F2021L00310:102 a legcons:Item,
        owl:Class,
        dcat:Resource ;
    rdfs:label "Item - I102 5 20  Prescribed poultry meat or poultry meat products for further processing"@en-AU ;
    dct:isPartOf F2021L00310:99 ;
    dct:isReferencedBy F2021L00310: ;
    rdfs:comment "5 20  Prescribed poultry meat or poultry meat products for further processing - Abrievated Graph Key: I102"@en-AU ;
    skos:definition "5 20  Prescribed poultry meat or poultry meat products for further processing"@en-AU ;
    skos:narrower F2021L00310:99 ;
    skos:prefLabel "Item I102"@en-AU ;
    dcat:accessURL <https://www.legislation.gov.au/F2021L00310/2023-08-04/2023-08-04/text/1/epub/OEBPS/document_1/document_1.html#_Toc145601428> ;
    dcat:landingPage "https://www.legislation.gov.au/F2021L00310/2023-08-04/2023-08-04/text/1/epub/OEBPS/document_1/document_1.html#_Toc145601428"^^xsd:anyURI ;
    dcat:theme legcons:Item .

F2021L00310:104 a legcons:Item,
        owl:Class,
        dcat:Resource ;
    rdfs:label "Item - I104 5 21  References to particular official marks"@en-AU ;
    dct:isPartOf F2021L00310:103 ;
    dct:isReferencedBy F2021L00310: ;
    rdfs:comment "5 21  References to particular official marks - Abrievated Graph Key: I104"@en-AU ;
    skos:definition "5 21  References to particular official marks"@en-AU ;
    skos:narrower F2021L00310:103 ;
    skos:prefLabel "Item I104"@en-AU ;
    dcat:accessURL <https://www.legislation.gov.au/F2021L00310/2023-08-04/2023-08-04/text/1/epub/OEBPS/document_1/document_1.html#_Toc145601430> ;
    dcat:landingPage "https://www.legislation.gov.au/F2021L00310/2023-08-04/2023-08-04/text/1/epub/OEBPS/document_1/document_1.html#_Toc145601430"^^xsd:anyURI ;
    dcat:theme legcons:Item .

F2021L00310:105 a legcons:Item,
        owl:Class,
        dcat:Resource ;
    rdfs:label "Item - I105 5 22  Cartons containing prescribed poultry meat or poultry meat products"@en-AU ;
    dct:isPartOf F2021L00310:103 ;
    dct:isReferencedBy F2021L00310: ;
    rdfs:comment "5 22  Cartons containing prescribed poultry meat or poultry meat products - Abrievated Graph Key: I105"@en-AU ;
    skos:definition "5 22  Cartons containing prescribed poultry meat or poultry meat products"@en-AU ;
    skos:narrower F2021L00310:103 ;
    skos:prefLabel "Item I105"@en-AU ;
    dcat:accessURL <https://www.legislation.gov.au/F2021L00310/2023-08-04/2023-08-04/text/1/epub/OEBPS/document_1/document_1.html#_Toc145601431> ;
    dcat:landingPage "https://www.legislation.gov.au/F2021L00310/2023-08-04/2023-08-04/text/1/epub/OEBPS/document_1/document_1.html#_Toc145601431"^^xsd:anyURI ;
    dcat:theme legcons:Item .

F2021L00310:106 a legcons:Item,
        owl:Class,
        dcat:Resource ;
    rdfs:label "Item - I106 5 23  Other applications of official mark to prescribed poultry meat or poultry meat products"@en-AU ;
    dct:isPartOf F2021L00310:103 ;
    dct:isReferencedBy F2021L00310: ;
    rdfs:comment "5 23  Other applications of official mark to prescribed poultry meat or poultry meat products - Abrievated Graph Key: I106"@en-AU ;
    skos:definition "5 23  Other applications of official mark to prescribed poultry meat or poultry meat products"@en-AU ;
    skos:narrower F2021L00310:103 ;
    skos:prefLabel "Item I106"@en-AU ;
    dcat:accessURL <https://www.legislation.gov.au/F2021L00310/2023-08-04/2023-08-04/text/1/epub/OEBPS/document_1/document_1.html#_Toc145601432> ;
    dcat:landingPage "https://www.legislation.gov.au/F2021L00310/2023-08-04/2023-08-04/text/1/epub/OEBPS/document_1/document_1.html#_Toc145601432"^^xsd:anyURI ;
    dcat:theme legcons:Item .

F2021L00310:107 a legcons:Item,
        owl:Class,
        dcat:Resource ;
    rdfs:label "Item - I107 5 24  State or Territory classification marks must not be applied"@en-AU ;
    dct:isPartOf F2021L00310:103 ;
    dct:isReferencedBy F2021L00310: ;
    rdfs:comment "5 24  State or Territory classification marks must not be applied - Abrievated Graph Key: I107"@en-AU ;
    skos:definition "5 24  State or Territory classification marks must not be applied"@en-AU ;
    skos:narrower F2021L00310:103 ;
    skos:prefLabel "Item I107"@en-AU ;
    dcat:accessURL <https://www.legislation.gov.au/F2021L00310/2023-08-04/2023-08-04/text/1/epub/OEBPS/document_1/document_1.html#_Toc145601433> ;
    dcat:landingPage "https://www.legislation.gov.au/F2021L00310/2023-08-04/2023-08-04/text/1/epub/OEBPS/document_1/document_1.html#_Toc145601433"^^xsd:anyURI ;
    dcat:theme legcons:Item .

F2021L00310:109 a legcons:Item,
        owl:Class,
        dcat:Resource ;
    rdfs:label "Item - I109 5 25  Segregation identification security and traceabilitygeneral"@en-AU ;
    dct:isPartOf F2021L00310:108 ;
    dct:isReferencedBy F2021L00310: ;
    rdfs:comment "5 25  Segregation identification security and traceabilitygeneral - Abrievated Graph Key: I109"@en-AU ;
    skos:definition "5 25  Segregation identification security and traceabilitygeneral"@en-AU ;
    skos:narrower F2021L00310:108 ;
    skos:prefLabel "Item I109"@en-AU ;
    dcat:accessURL <https://www.legislation.gov.au/F2021L00310/2023-08-04/2023-08-04/text/1/epub/OEBPS/document_1/document_1.html#_Toc145601435> ;
    dcat:landingPage "https://www.legislation.gov.au/F2021L00310/2023-08-04/2023-08-04/text/1/epub/OEBPS/document_1/document_1.html#_Toc145601435"^^xsd:anyURI ;
    dcat:theme legcons:Item .

F2021L00310:11 a legcons:Item,
        owl:Class,
        dcat:Resource ;
    rdfs:label "Item - I11 1 7  Modifications of certain terms used in the Australian Poultry Meat Standard"@en-AU ;
    dct:isPartOf F2021L00310:1 ;
    dct:isReferencedBy F2021L00310: ;
    rdfs:comment "1 7  Modifications of certain terms used in the Australian Poultry Meat Standard - Abrievated Graph Key: I11"@en-AU ;
    skos:definition "1 7  Modifications of certain terms used in the Australian Poultry Meat Standard"@en-AU ;
    skos:narrower F2021L00310:1 ;
    skos:prefLabel "Item I11"@en-AU ;
    dcat:accessURL <https://www.legislation.gov.au/F2021L00310/2023-08-04/2023-08-04/text/1/epub/OEBPS/document_1/document_1.html#_Toc145601337> ;
    dcat:landingPage "https://www.legislation.gov.au/F2021L00310/2023-08-04/2023-08-04/text/1/epub/OEBPS/document_1/document_1.html#_Toc145601337"^^xsd:anyURI ;
    dcat:theme legcons:Item .

F2021L00310:110 a legcons:Item,
        owl:Class,
        dcat:Resource ;
    rdfs:label "Item - I110 5 26  Establishments where poultry meat or poultry meat products that are not for export etc are prepared"@en-AU ;
    dct:isPartOf F2021L00310:108 ;
    dct:isReferencedBy F2021L00310: ;
    rdfs:comment "5 26  Establishments where poultry meat or poultry meat products that are not for export etc are prepared - Abrievated Graph Key: I110"@en-AU ;
    skos:definition "5 26  Establishments where poultry meat or poultry meat products that are not for export etc are prepared"@en-AU ;
    skos:narrower F2021L00310:108 ;
    skos:prefLabel "Item I110"@en-AU ;
    dcat:accessURL <https://www.legislation.gov.au/F2021L00310/2023-08-04/2023-08-04/text/1/epub/OEBPS/document_1/document_1.html#_Toc145601436> ;
    dcat:landingPage "https://www.legislation.gov.au/F2021L00310/2023-08-04/2023-08-04/text/1/epub/OEBPS/document_1/document_1.html#_Toc145601436"^^xsd:anyURI ;
    dcat:theme legcons:Item .

F2021L00310:111 a legcons:Item,
        owl:Class,
        dcat:Resource ;
    rdfs:label "Item - I111 5 27  Integritygeneral"@en-AU ;
    dct:isPartOf F2021L00310:108 ;
    dct:isReferencedBy F2021L00310: ;
    rdfs:comment "5 27  Integritygeneral - Abrievated Graph Key: I111"@en-AU ;
    skos:definition "5 27  Integritygeneral"@en-AU ;
    skos:narrower F2021L00310:108 ;
    skos:prefLabel "Item I111"@en-AU ;
    dcat:accessURL <https://www.legislation.gov.au/F2021L00310/2023-08-04/2023-08-04/text/1/epub/OEBPS/document_1/document_1.html#_Toc145601437> ;
    dcat:landingPage "https://www.legislation.gov.au/F2021L00310/2023-08-04/2023-08-04/text/1/epub/OEBPS/document_1/document_1.html#_Toc145601437"^^xsd:anyURI ;
    dcat:theme legcons:Item .

F2021L00310:112 a legcons:Item,
        owl:Class,
        dcat:Resource ;
    rdfs:label "Item - I112 5 28  Identificationtype of poultry"@en-AU ;
    dct:isPartOf F2021L00310:108 ;
    dct:isReferencedBy F2021L00310: ;
    rdfs:comment "5 28  Identificationtype of poultry - Abrievated Graph Key: I112"@en-AU ;
    skos:definition "5 28  Identificationtype of poultry"@en-AU ;
    skos:narrower F2021L00310:108 ;
    skos:prefLabel "Item I112"@en-AU ;
    dcat:accessURL <https://www.legislation.gov.au/F2021L00310/2023-08-04/2023-08-04/text/1/epub/OEBPS/document_1/document_1.html#_Toc145601438> ;
    dcat:landingPage "https://www.legislation.gov.au/F2021L00310/2023-08-04/2023-08-04/text/1/epub/OEBPS/document_1/document_1.html#_Toc145601438"^^xsd:anyURI ;
    dcat:theme legcons:Item .

F2021L00310:113 a legcons:Item,
        owl:Class,
        dcat:Resource ;
    rdfs:label "Item - I113 5 29  Export market eligibility"@en-AU ;
    dct:isPartOf F2021L00310:108 ;
    dct:isReferencedBy F2021L00310: ;
    rdfs:comment "5 29  Export market eligibility - Abrievated Graph Key: I113"@en-AU ;
    skos:definition "5 29  Export market eligibility"@en-AU ;
    skos:narrower F2021L00310:108 ;
    skos:prefLabel "Item I113"@en-AU ;
    dcat:accessURL <https://www.legislation.gov.au/F2021L00310/2023-08-04/2023-08-04/text/1/epub/OEBPS/document_1/document_1.html#_Toc145601439> ;
    dcat:landingPage "https://www.legislation.gov.au/F2021L00310/2023-08-04/2023-08-04/text/1/epub/OEBPS/document_1/document_1.html#_Toc145601439"^^xsd:anyURI ;
    dcat:theme legcons:Item .

F2021L00310:114 a legcons:Item,
        owl:Class,
        dcat:Resource ;
    rdfs:label "Item - I114 5 30  Action if prescribed poultry meat or poultry meat products are unwholesome or integrity etc cannot be ensured"@en-AU ;
    dct:isPartOf F2021L00310:108 ;
    dct:isReferencedBy F2021L00310: ;
    rdfs:comment "5 30  Action if prescribed poultry meat or poultry meat products are unwholesome or integrity etc cannot be ensured - Abrievated Graph Key: I114"@en-AU ;
    skos:definition "5 30  Action if prescribed poultry meat or poultry meat products are unwholesome or integrity etc cannot be ensured"@en-AU ;
    skos:narrower F2021L00310:108 ;
    skos:prefLabel "Item I114"@en-AU ;
    dcat:accessURL <https://www.legislation.gov.au/F2021L00310/2023-08-04/2023-08-04/text/1/epub/OEBPS/document_1/document_1.html#_Toc145601440> ;
    dcat:landingPage "https://www.legislation.gov.au/F2021L00310/2023-08-04/2023-08-04/text/1/epub/OEBPS/document_1/document_1.html#_Toc145601440"^^xsd:anyURI ;
    dcat:theme legcons:Item .

F2021L00310:116 a legcons:Item,
        owl:Class,
        dcat:Resource ;
    rdfs:label "Item - I116 5 31  Information and declarations relating to transferred prescribed poultry meat or poultry meat products"@en-AU ;
    dct:isPartOf F2021L00310:115 ;
    dct:isReferencedBy F2021L00310: ;
    rdfs:comment "5 31  Information and declarations relating to transferred prescribed poultry meat or poultry meat products - Abrievated Graph Key: I116"@en-AU ;
    skos:definition "5 31  Information and declarations relating to transferred prescribed poultry meat or poultry meat products"@en-AU ;
    skos:narrower F2021L00310:115 ;
    skos:prefLabel "Item I116"@en-AU ;
    dcat:accessURL <https://www.legislation.gov.au/F2021L00310/2023-08-04/2023-08-04/text/1/epub/OEBPS/document_1/document_1.html#_Toc145601442> ;
    dcat:landingPage "https://www.legislation.gov.au/F2021L00310/2023-08-04/2023-08-04/text/1/epub/OEBPS/document_1/document_1.html#_Toc145601442"^^xsd:anyURI ;
    dcat:theme legcons:Item .

F2021L00310:117 a legcons:Item,
        owl:Class,
        dcat:Resource ;
    rdfs:label "Item - I117 5 32  Information and declarations not received or inaccurate or incomplete"@en-AU ;
    dct:isPartOf F2021L00310:115 ;
    dct:isReferencedBy F2021L00310: ;
    rdfs:comment "5 32  Information and declarations not received or inaccurate or incomplete - Abrievated Graph Key: I117"@en-AU ;
    skos:definition "5 32  Information and declarations not received or inaccurate or incomplete"@en-AU ;
    skos:narrower F2021L00310:115 ;
    skos:prefLabel "Item I117"@en-AU ;
    dcat:accessURL <https://www.legislation.gov.au/F2021L00310/2023-08-04/2023-08-04/text/1/epub/OEBPS/document_1/document_1.html#_Toc145601443> ;
    dcat:landingPage "https://www.legislation.gov.au/F2021L00310/2023-08-04/2023-08-04/text/1/epub/OEBPS/document_1/document_1.html#_Toc145601443"^^xsd:anyURI ;
    dcat:theme legcons:Item .

F2021L00310:119 a legcons:Item,
        owl:Class,
        dcat:Resource ;
    rdfs:label "Item - I119 5 33  Authorised officer must be present while certain export operations are carried out"@en-AU ;
    dct:isPartOf F2021L00310:118 ;
    dct:isReferencedBy F2021L00310: ;
    rdfs:comment "5 33  Authorised officer must be present while certain export operations are carried out - Abrievated Graph Key: I119"@en-AU ;
    skos:definition "5 33  Authorised officer must be present while certain export operations are carried out"@en-AU ;
    skos:narrower F2021L00310:118 ;
    skos:prefLabel "Item I119"@en-AU ;
    dcat:accessURL <https://www.legislation.gov.au/F2021L00310/2023-08-04/2023-08-04/text/1/epub/OEBPS/document_1/document_1.html#_Toc145601445> ;
    dcat:landingPage "https://www.legislation.gov.au/F2021L00310/2023-08-04/2023-08-04/text/1/epub/OEBPS/document_1/document_1.html#_Toc145601445"^^xsd:anyURI ;
    dcat:theme legcons:Item .

F2021L00310:12 a legcons:Item,
        owl:Class,
        dcat:Resource ;
    rdfs:label "Item - I12 1 8  Circumstances in which alternative procedure standard or other requirement is taken to meet requirements of Australian Poultry Meat Standard"@en-AU ;
    dct:isPartOf F2021L00310:1 ;
    dct:isReferencedBy F2021L00310: ;
    rdfs:comment "1 8  Circumstances in which alternative procedure standard or other requirement is taken to meet requirements of Australian Poultry Meat Standard - Abrievated Graph Key: I12"@en-AU ;
    skos:definition "1 8  Circumstances in which alternative procedure standard or other requirement is taken to meet requirements of Australian Poultry Meat Standard"@en-AU ;
    skos:narrower F2021L00310:1 ;
    skos:prefLabel "Item I12"@en-AU ;
    dcat:accessURL <https://www.legislation.gov.au/F2021L00310/2023-08-04/2023-08-04/text/1/epub/OEBPS/document_1/document_1.html#_Toc145601338> ;
    dcat:landingPage "https://www.legislation.gov.au/F2021L00310/2023-08-04/2023-08-04/text/1/epub/OEBPS/document_1/document_1.html#_Toc145601338"^^xsd:anyURI ;
    dcat:theme legcons:Item .

F2021L00310:121 a legcons:Item,
        owl:Class,
        dcat:Resource ;
    rdfs:label "Item - I121 5 34  Management practices organisational structure resources and personnel"@en-AU ;
    dct:isPartOf F2021L00310:120 ;
    dct:isReferencedBy F2021L00310: ;
    rdfs:comment "5 34  Management practices organisational structure resources and personnel - Abrievated Graph Key: I121"@en-AU ;
    skos:definition "5 34  Management practices organisational structure resources and personnel"@en-AU ;
    skos:narrower F2021L00310:120 ;
    skos:prefLabel "Item I121"@en-AU ;
    dcat:accessURL <https://www.legislation.gov.au/F2021L00310/2023-08-04/2023-08-04/text/1/epub/OEBPS/document_1/document_1.html#_Toc145601447> ;
    dcat:landingPage "https://www.legislation.gov.au/F2021L00310/2023-08-04/2023-08-04/text/1/epub/OEBPS/document_1/document_1.html#_Toc145601447"^^xsd:anyURI ;
    dcat:theme legcons:Item .

F2021L00310:122 a legcons:Item,
        owl:Class,
        dcat:Resource ;
    rdfs:label "Item - I122 5 35  Verification of compliance with the Act and other matters"@en-AU ;
    dct:isPartOf F2021L00310:120 ;
    dct:isReferencedBy F2021L00310: ;
    rdfs:comment "5 35  Verification of compliance with the Act and other matters - Abrievated Graph Key: I122"@en-AU ;
    skos:definition "5 35  Verification of compliance with the Act and other matters"@en-AU ;
    skos:narrower F2021L00310:120 ;
    skos:prefLabel "Item I122"@en-AU ;
    dcat:accessURL <https://www.legislation.gov.au/F2021L00310/2023-08-04/2023-08-04/text/1/epub/OEBPS/document_1/document_1.html#_Toc145601448> ;
    dcat:landingPage "https://www.legislation.gov.au/F2021L00310/2023-08-04/2023-08-04/text/1/epub/OEBPS/document_1/document_1.html#_Toc145601448"^^xsd:anyURI ;
    dcat:theme legcons:Item .

F2021L00310:123 a legcons:Item,
        owl:Class,
        dcat:Resource ;
    rdfs:label "Item - I123 5 36  Action must be taken to address non compliance"@en-AU ;
    dct:isPartOf F2021L00310:120 ;
    dct:isReferencedBy F2021L00310: ;
    rdfs:comment "5 36  Action must be taken to address non compliance - Abrievated Graph Key: I123"@en-AU ;
    skos:definition "5 36  Action must be taken to address non compliance"@en-AU ;
    skos:narrower F2021L00310:120 ;
    skos:prefLabel "Item I123"@en-AU ;
    dcat:accessURL <https://www.legislation.gov.au/F2021L00310/2023-08-04/2023-08-04/text/1/epub/OEBPS/document_1/document_1.html#_Toc145601449> ;
    dcat:landingPage "https://www.legislation.gov.au/F2021L00310/2023-08-04/2023-08-04/text/1/epub/OEBPS/document_1/document_1.html#_Toc145601449"^^xsd:anyURI ;
    dcat:theme legcons:Item .

F2021L00310:124 a legcons:Item,
        owl:Class,
        dcat:Resource ;
    rdfs:label "Item - I124 5 37  Internal audit and management review"@en-AU ;
    dct:isPartOf F2021L00310:120 ;
    dct:isReferencedBy F2021L00310: ;
    rdfs:comment "5 37  Internal audit and management review - Abrievated Graph Key: I124"@en-AU ;
    skos:definition "5 37  Internal audit and management review"@en-AU ;
    skos:narrower F2021L00310:120 ;
    skos:prefLabel "Item I124"@en-AU ;
    dcat:accessURL <https://www.legislation.gov.au/F2021L00310/2023-08-04/2023-08-04/text/1/epub/OEBPS/document_1/document_1.html#_Toc145601450> ;
    dcat:landingPage "https://www.legislation.gov.au/F2021L00310/2023-08-04/2023-08-04/text/1/epub/OEBPS/document_1/document_1.html#_Toc145601450"^^xsd:anyURI ;
    dcat:theme legcons:Item .

F2021L00310:126 a legcons:Item,
        owl:Class,
        dcat:Resource ;
    rdfs:label "Item - I126 5 38  Period within which application to renew approved arrangement must be made"@en-AU ;
    dct:isPartOf F2021L00310:125 ;
    dct:isReferencedBy F2021L00310: ;
    rdfs:comment "5 38  Period within which application to renew approved arrangement must be made - Abrievated Graph Key: I126"@en-AU ;
    skos:definition "5 38  Period within which application to renew approved arrangement must be made"@en-AU ;
    skos:narrower F2021L00310:125 ;
    skos:prefLabel "Item I126"@en-AU ;
    dcat:accessURL <https://www.legislation.gov.au/F2021L00310/2023-08-04/2023-08-04/text/1/epub/OEBPS/document_1/document_1.html#_Toc145601452> ;
    dcat:landingPage "https://www.legislation.gov.au/F2021L00310/2023-08-04/2023-08-04/text/1/epub/OEBPS/document_1/document_1.html#_Toc145601452"^^xsd:anyURI ;
    dcat:theme legcons:Item .

F2021L00310:129 a legcons:Item,
        owl:Class,
        dcat:Resource ;
    rdfs:label "Item - I129 5 39  Requirements that must be met for variation to be approved or conditions varied"@en-AU ;
    dct:isPartOf F2021L00310:128 ;
    dct:isReferencedBy F2021L00310: ;
    rdfs:comment "5 39  Requirements that must be met for variation to be approved or conditions varied - Abrievated Graph Key: I129"@en-AU ;
    skos:definition "5 39  Requirements that must be met for variation to be approved or conditions varied"@en-AU ;
    skos:narrower F2021L00310:128 ;
    skos:prefLabel "Item I129"@en-AU ;
    dcat:accessURL <https://www.legislation.gov.au/F2021L00310/2023-08-04/2023-08-04/text/1/epub/OEBPS/document_1/document_1.html#_Toc145601455> ;
    dcat:landingPage "https://www.legislation.gov.au/F2021L00310/2023-08-04/2023-08-04/text/1/epub/OEBPS/document_1/document_1.html#_Toc145601455"^^xsd:anyURI ;
    dcat:theme legcons:Item .

F2021L00310:130 a legcons:Item,
        owl:Class,
        dcat:Resource ;
    rdfs:label "Item - I130 5 40  Significant variations"@en-AU ;
    dct:isPartOf F2021L00310:128 ;
    dct:isReferencedBy F2021L00310: ;
    rdfs:comment "5 40  Significant variations - Abrievated Graph Key: I130"@en-AU ;
    skos:definition "5 40  Significant variations"@en-AU ;
    skos:narrower F2021L00310:128 ;
    skos:prefLabel "Item I130"@en-AU ;
    dcat:accessURL <https://www.legislation.gov.au/F2021L00310/2023-08-04/2023-08-04/text/1/epub/OEBPS/document_1/document_1.html#_Toc145601456> ;
    dcat:landingPage "https://www.legislation.gov.au/F2021L00310/2023-08-04/2023-08-04/text/1/epub/OEBPS/document_1/document_1.html#_Toc145601456"^^xsd:anyURI ;
    dcat:theme legcons:Item .

F2021L00310:132 a legcons:Item,
        owl:Class,
        dcat:Resource ;
    rdfs:label "Item - I132 5 41  Other reasons for requiring holder to vary approved arrangement"@en-AU ;
    dct:isPartOf F2021L00310:131 ;
    dct:isReferencedBy F2021L00310: ;
    rdfs:comment "5 41  Other reasons for requiring holder to vary approved arrangement - Abrievated Graph Key: I132"@en-AU ;
    skos:definition "5 41  Other reasons for requiring holder to vary approved arrangement"@en-AU ;
    skos:narrower F2021L00310:131 ;
    skos:prefLabel "Item I132"@en-AU ;
    dcat:accessURL <https://www.legislation.gov.au/F2021L00310/2023-08-04/2023-08-04/text/1/epub/OEBPS/document_1/document_1.html#_Toc145601458> ;
    dcat:landingPage "https://www.legislation.gov.au/F2021L00310/2023-08-04/2023-08-04/text/1/epub/OEBPS/document_1/document_1.html#_Toc145601458"^^xsd:anyURI ;
    dcat:theme legcons:Item .

F2021L00310:134 a legcons:Item,
        owl:Class,
        dcat:Resource ;
    rdfs:label "Item - I134 5 42  Application of this Part"@en-AU ;
    dct:isPartOf F2021L00310:133 ;
    dct:isReferencedBy F2021L00310: ;
    rdfs:comment "5 42  Application of this Part - Abrievated Graph Key: I134"@en-AU ;
    skos:definition "5 42  Application of this Part"@en-AU ;
    skos:narrower F2021L00310:133 ;
    skos:prefLabel "Item I134"@en-AU ;
    dcat:accessURL <https://www.legislation.gov.au/F2021L00310/2023-08-04/2023-08-04/text/1/epub/OEBPS/document_1/document_1.html#_Toc145601460> ;
    dcat:landingPage "https://www.legislation.gov.au/F2021L00310/2023-08-04/2023-08-04/text/1/epub/OEBPS/document_1/document_1.html#_Toc145601460"^^xsd:anyURI ;
    dcat:theme legcons:Item .

F2021L00310:135 a legcons:Item,
        owl:Class,
        dcat:Resource ;
    rdfs:label "Item - I135 5 43  Initial consideration period"@en-AU ;
    dct:isPartOf F2021L00310:133 ;
    dct:isReferencedBy F2021L00310: ;
    rdfs:comment "5 43  Initial consideration period - Abrievated Graph Key: I135"@en-AU ;
    skos:definition "5 43  Initial consideration period"@en-AU ;
    skos:narrower F2021L00310:133 ;
    skos:prefLabel "Item I135"@en-AU ;
    dcat:accessURL <https://www.legislation.gov.au/F2021L00310/2023-08-04/2023-08-04/text/1/epub/OEBPS/document_1/document_1.html#_Toc145601461> ;
    dcat:landingPage "https://www.legislation.gov.au/F2021L00310/2023-08-04/2023-08-04/text/1/epub/OEBPS/document_1/document_1.html#_Toc145601461"^^xsd:anyURI ;
    dcat:theme legcons:Item .

F2021L00310:136 a legcons:Item,
        owl:Class,
        dcat:Resource ;
    rdfs:label "Item - I136 5 44  Period within which request relating to application must be complied with"@en-AU ;
    dct:isPartOf F2021L00310:133 ;
    dct:isReferencedBy F2021L00310: ;
    rdfs:comment "5 44  Period within which request relating to application must be complied with - Abrievated Graph Key: I136"@en-AU ;
    skos:definition "5 44  Period within which request relating to application must be complied with"@en-AU ;
    skos:narrower F2021L00310:133 ;
    skos:prefLabel "Item I136"@en-AU ;
    dcat:accessURL <https://www.legislation.gov.au/F2021L00310/2023-08-04/2023-08-04/text/1/epub/OEBPS/document_1/document_1.html#_Toc145601462> ;
    dcat:landingPage "https://www.legislation.gov.au/F2021L00310/2023-08-04/2023-08-04/text/1/epub/OEBPS/document_1/document_1.html#_Toc145601462"^^xsd:anyURI ;
    dcat:theme legcons:Item .

F2021L00310:139 a legcons:Item,
        owl:Class,
        dcat:Resource ;
    rdfs:label "Item - I139 7 1  Period of effect of export permit"@en-AU ;
    dct:isPartOf F2021L00310:138 ;
    dct:isReferencedBy F2021L00310: ;
    rdfs:comment "7 1  Period of effect of export permit - Abrievated Graph Key: I139"@en-AU ;
    skos:definition "7 1  Period of effect of export permit"@en-AU ;
    skos:narrower F2021L00310:138 ;
    skos:prefLabel "Item I139"@en-AU ;
    dcat:accessURL <https://www.legislation.gov.au/F2021L00310/2023-08-04/2023-08-04/text/1/epub/OEBPS/document_1/document_1.html#_Toc145601465> ;
    dcat:landingPage "https://www.legislation.gov.au/F2021L00310/2023-08-04/2023-08-04/text/1/epub/OEBPS/document_1/document_1.html#_Toc145601465"^^xsd:anyURI ;
    dcat:theme legcons:Item .

F2021L00310:141 a legcons:Item,
        owl:Class,
        dcat:Resource ;
    rdfs:label "Item - I141 7 2  Period of effect of varied export permit"@en-AU ;
    dct:isPartOf F2021L00310:140 ;
    dct:isReferencedBy F2021L00310: ;
    rdfs:comment "7 2  Period of effect of varied export permit - Abrievated Graph Key: I141"@en-AU ;
    skos:definition "7 2  Period of effect of varied export permit"@en-AU ;
    skos:narrower F2021L00310:140 ;
    skos:prefLabel "Item I141"@en-AU ;
    dcat:accessURL <https://www.legislation.gov.au/F2021L00310/2023-08-04/2023-08-04/text/1/epub/OEBPS/document_1/document_1.html#_Toc145601467> ;
    dcat:landingPage "https://www.legislation.gov.au/F2021L00310/2023-08-04/2023-08-04/text/1/epub/OEBPS/document_1/document_1.html#_Toc145601467"^^xsd:anyURI ;
    dcat:theme legcons:Item .

F2021L00310:142 a legcons:Item,
        owl:Class,
        dcat:Resource ;
    rdfs:label "Item - I142 7 3  Circumstances in which export permit may be suspended"@en-AU ;
    dct:isPartOf F2021L00310:140 ;
    dct:isReferencedBy F2021L00310: ;
    rdfs:comment "7 3  Circumstances in which export permit may be suspended - Abrievated Graph Key: I142"@en-AU ;
    skos:definition "7 3  Circumstances in which export permit may be suspended"@en-AU ;
    skos:narrower F2021L00310:140 ;
    skos:prefLabel "Item I142"@en-AU ;
    dcat:accessURL <https://www.legislation.gov.au/F2021L00310/2023-08-04/2023-08-04/text/1/epub/OEBPS/document_1/document_1.html#_Toc145601468> ;
    dcat:landingPage "https://www.legislation.gov.au/F2021L00310/2023-08-04/2023-08-04/text/1/epub/OEBPS/document_1/document_1.html#_Toc145601468"^^xsd:anyURI ;
    dcat:theme legcons:Item .

F2021L00310:143 a legcons:Item,
        owl:Class,
        dcat:Resource ;
    rdfs:label "Item - I143 7 4  Other circumstances in which export permit may be revoked"@en-AU ;
    dct:isPartOf F2021L00310:140 ;
    dct:isReferencedBy F2021L00310: ;
    rdfs:comment "7 4  Other circumstances in which export permit may be revoked - Abrievated Graph Key: I143"@en-AU ;
    skos:definition "7 4  Other circumstances in which export permit may be revoked"@en-AU ;
    skos:narrower F2021L00310:140 ;
    skos:prefLabel "Item I143"@en-AU ;
    dcat:accessURL <https://www.legislation.gov.au/F2021L00310/2023-08-04/2023-08-04/text/1/epub/OEBPS/document_1/document_1.html#_Toc145601469> ;
    dcat:landingPage "https://www.legislation.gov.au/F2021L00310/2023-08-04/2023-08-04/text/1/epub/OEBPS/document_1/document_1.html#_Toc145601469"^^xsd:anyURI ;
    dcat:theme legcons:Item .

F2021L00310:145 a legcons:Item,
        owl:Class,
        dcat:Resource ;
    rdfs:label "Item - I145 7 5  Changes that require additional or corrected information to be given to the Secretary"@en-AU ;
    dct:isPartOf F2021L00310:144 ;
    dct:isReferencedBy F2021L00310: ;
    rdfs:comment "7 5  Changes that require additional or corrected information to be given to the Secretary - Abrievated Graph Key: I145"@en-AU ;
    skos:definition "7 5  Changes that require additional or corrected information to be given to the Secretary"@en-AU ;
    skos:narrower F2021L00310:144 ;
    skos:prefLabel "Item I145"@en-AU ;
    dcat:accessURL <https://www.legislation.gov.au/F2021L00310/2023-08-04/2023-08-04/text/1/epub/OEBPS/document_1/document_1.html#_Toc145601471> ;
    dcat:landingPage "https://www.legislation.gov.au/F2021L00310/2023-08-04/2023-08-04/text/1/epub/OEBPS/document_1/document_1.html#_Toc145601471"^^xsd:anyURI ;
    dcat:theme legcons:Item .

F2021L00310:146 a legcons:Item,
        owl:Class,
        dcat:Resource ;
    rdfs:label "Item - I146 7 6  Return of export permit"@en-AU ;
    dct:isPartOf F2021L00310:144 ;
    dct:isReferencedBy F2021L00310: ;
    rdfs:comment "7 6  Return of export permit - Abrievated Graph Key: I146"@en-AU ;
    skos:definition "7 6  Return of export permit"@en-AU ;
    skos:narrower F2021L00310:144 ;
    skos:prefLabel "Item I146"@en-AU ;
    dcat:accessURL <https://www.legislation.gov.au/F2021L00310/2023-08-04/2023-08-04/text/1/epub/OEBPS/document_1/document_1.html#_Toc145601472> ;
    dcat:landingPage "https://www.legislation.gov.au/F2021L00310/2023-08-04/2023-08-04/text/1/epub/OEBPS/document_1/document_1.html#_Toc145601472"^^xsd:anyURI ;
    dcat:theme legcons:Item .

F2021L00310:147 a legcons:Item,
        owl:Class,
        dcat:Resource ;
    rdfs:label "Item - I147 7 7  Notification that prescribed poultry meat or poultry meat products are not to be exported"@en-AU ;
    dct:isPartOf F2021L00310:144 ;
    dct:isReferencedBy F2021L00310: ;
    rdfs:comment "7 7  Notification that prescribed poultry meat or poultry meat products are not to be exported - Abrievated Graph Key: I147"@en-AU ;
    skos:definition "7 7  Notification that prescribed poultry meat or poultry meat products are not to be exported"@en-AU ;
    skos:narrower F2021L00310:144 ;
    skos:prefLabel "Item I147"@en-AU ;
    dcat:accessURL <https://www.legislation.gov.au/F2021L00310/2023-08-04/2023-08-04/text/1/epub/OEBPS/document_1/document_1.html#_Toc145601473> ;
    dcat:landingPage "https://www.legislation.gov.au/F2021L00310/2023-08-04/2023-08-04/text/1/epub/OEBPS/document_1/document_1.html#_Toc145601473"^^xsd:anyURI ;
    dcat:theme legcons:Item .

F2021L00310:148 a legcons:Item,
        owl:Class,
        dcat:Resource ;
    rdfs:label "Item - I148 7 8  Application for export permit must include declaration"@en-AU ;
    dct:isPartOf F2021L00310:144 ;
    dct:isReferencedBy F2021L00310: ;
    rdfs:comment "7 8  Application for export permit must include declaration - Abrievated Graph Key: I148"@en-AU ;
    skos:definition "7 8  Application for export permit must include declaration"@en-AU ;
    skos:narrower F2021L00310:144 ;
    skos:prefLabel "Item I148"@en-AU ;
    dcat:accessURL <https://www.legislation.gov.au/F2021L00310/2023-08-04/2023-08-04/text/1/epub/OEBPS/document_1/document_1.html#_Toc145601474> ;
    dcat:landingPage "https://www.legislation.gov.au/F2021L00310/2023-08-04/2023-08-04/text/1/epub/OEBPS/document_1/document_1.html#_Toc145601474"^^xsd:anyURI ;
    dcat:theme legcons:Item .

F2021L00310:151 a legcons:Item,
        owl:Class,
        dcat:Resource ;
    rdfs:label "Item - I151 8 1  Information to be included in notice of intention to export"@en-AU ;
    dct:isPartOf F2021L00310:150 ;
    dct:isReferencedBy F2021L00310: ;
    rdfs:comment "8 1  Information to be included in notice of intention to export - Abrievated Graph Key: I151"@en-AU ;
    skos:definition "8 1  Information to be included in notice of intention to export"@en-AU ;
    skos:narrower F2021L00310:150 ;
    skos:prefLabel "Item I151"@en-AU ;
    dcat:accessURL <https://www.legislation.gov.au/F2021L00310/2023-08-04/2023-08-04/text/1/epub/OEBPS/document_1/document_1.html#_Toc145601477> ;
    dcat:landingPage "https://www.legislation.gov.au/F2021L00310/2023-08-04/2023-08-04/text/1/epub/OEBPS/document_1/document_1.html#_Toc145601477"^^xsd:anyURI ;
    dcat:theme legcons:Item .

F2021L00310:152 a legcons:Item,
        owl:Class,
        dcat:Resource ;
    rdfs:label "Item - I152 8 2  Person who must give notice of intention to export"@en-AU ;
    dct:isPartOf F2021L00310:150 ;
    dct:isReferencedBy F2021L00310: ;
    rdfs:comment "8 2  Person who must give notice of intention to export - Abrievated Graph Key: I152"@en-AU ;
    skos:definition "8 2  Person who must give notice of intention to export"@en-AU ;
    skos:narrower F2021L00310:150 ;
    skos:prefLabel "Item I152"@en-AU ;
    dcat:accessURL <https://www.legislation.gov.au/F2021L00310/2023-08-04/2023-08-04/text/1/epub/OEBPS/document_1/document_1.html#_Toc145601478> ;
    dcat:landingPage "https://www.legislation.gov.au/F2021L00310/2023-08-04/2023-08-04/text/1/epub/OEBPS/document_1/document_1.html#_Toc145601478"^^xsd:anyURI ;
    dcat:theme legcons:Item .

F2021L00310:153 a legcons:Item,
        owl:Class,
        dcat:Resource ;
    rdfs:label "Item - I153 8 3  Person to whom notice of intention to export must be given"@en-AU ;
    dct:isPartOf F2021L00310:150 ;
    dct:isReferencedBy F2021L00310: ;
    rdfs:comment "8 3  Person to whom notice of intention to export must be given - Abrievated Graph Key: I153"@en-AU ;
    skos:definition "8 3  Person to whom notice of intention to export must be given"@en-AU ;
    skos:narrower F2021L00310:150 ;
    skos:prefLabel "Item I153"@en-AU ;
    dcat:accessURL <https://www.legislation.gov.au/F2021L00310/2023-08-04/2023-08-04/text/1/epub/OEBPS/document_1/document_1.html#_Toc145601479> ;
    dcat:landingPage "https://www.legislation.gov.au/F2021L00310/2023-08-04/2023-08-04/text/1/epub/OEBPS/document_1/document_1.html#_Toc145601479"^^xsd:anyURI ;
    dcat:theme legcons:Item .

F2021L00310:154 a legcons:Item,
        owl:Class,
        dcat:Resource ;
    rdfs:label "Item - I154 8 4  When notice of intention to export must be given"@en-AU ;
    dct:isPartOf F2021L00310:150 ;
    dct:isReferencedBy F2021L00310: ;
    rdfs:comment "8 4  When notice of intention to export must be given - Abrievated Graph Key: I154"@en-AU ;
    skos:definition "8 4  When notice of intention to export must be given"@en-AU ;
    skos:narrower F2021L00310:150 ;
    skos:prefLabel "Item I154"@en-AU ;
    dcat:accessURL <https://www.legislation.gov.au/F2021L00310/2023-08-04/2023-08-04/text/1/epub/OEBPS/document_1/document_1.html#_Toc145601480> ;
    dcat:landingPage "https://www.legislation.gov.au/F2021L00310/2023-08-04/2023-08-04/text/1/epub/OEBPS/document_1/document_1.html#_Toc145601480"^^xsd:anyURI ;
    dcat:theme legcons:Item .

F2021L00310:156 a legcons:Item,
        owl:Class,
        dcat:Resource ;
    rdfs:label "Item - I156 8 5  Purpose of this Part"@en-AU ;
    dct:isPartOf F2021L00310:155 ;
    dct:isReferencedBy F2021L00310: ;
    rdfs:comment "8 5  Purpose of this Part - Abrievated Graph Key: I156"@en-AU ;
    skos:definition "8 5  Purpose of this Part"@en-AU ;
    skos:narrower F2021L00310:155 ;
    skos:prefLabel "Item I156"@en-AU ;
    dcat:accessURL <https://www.legislation.gov.au/F2021L00310/2023-08-04/2023-08-04/text/1/epub/OEBPS/document_1/document_1.html#_Toc145601482> ;
    dcat:landingPage "https://www.legislation.gov.au/F2021L00310/2023-08-04/2023-08-04/text/1/epub/OEBPS/document_1/document_1.html#_Toc145601482"^^xsd:anyURI ;
    dcat:theme legcons:Item .

F2021L00310:157 a legcons:Item,
        owl:Class,
        dcat:Resource ;
    rdfs:label "Item - I157 8 6  General requirements for trade descriptions"@en-AU ;
    dct:isPartOf F2021L00310:155 ;
    dct:isReferencedBy F2021L00310: ;
    rdfs:comment "8 6  General requirements for trade descriptions - Abrievated Graph Key: I157"@en-AU ;
    skos:definition "8 6  General requirements for trade descriptions"@en-AU ;
    skos:narrower F2021L00310:155 ;
    skos:prefLabel "Item I157"@en-AU ;
    dcat:accessURL <https://www.legislation.gov.au/F2021L00310/2023-08-04/2023-08-04/text/1/epub/OEBPS/document_1/document_1.html#_Toc145601483> ;
    dcat:landingPage "https://www.legislation.gov.au/F2021L00310/2023-08-04/2023-08-04/text/1/epub/OEBPS/document_1/document_1.html#_Toc145601483"^^xsd:anyURI ;
    dcat:theme legcons:Item .

F2021L00310:158 a legcons:Item,
        owl:Class,
        dcat:Resource ;
    rdfs:label "Item - I158 8 7  Trade descriptions in language other than English"@en-AU ;
    dct:isPartOf F2021L00310:155 ;
    dct:isReferencedBy F2021L00310: ;
    rdfs:comment "8 7  Trade descriptions in language other than English - Abrievated Graph Key: I158"@en-AU ;
    skos:definition "8 7  Trade descriptions in language other than English"@en-AU ;
    skos:narrower F2021L00310:155 ;
    skos:prefLabel "Item I158"@en-AU ;
    dcat:accessURL <https://www.legislation.gov.au/F2021L00310/2023-08-04/2023-08-04/text/1/epub/OEBPS/document_1/document_1.html#_Toc145601484> ;
    dcat:landingPage "https://www.legislation.gov.au/F2021L00310/2023-08-04/2023-08-04/text/1/epub/OEBPS/document_1/document_1.html#_Toc145601484"^^xsd:anyURI ;
    dcat:theme legcons:Item .

F2021L00310:16 a legcons:Item,
        owl:Class,
        dcat:Resource ;
    rdfs:label "Item - I16 2 1  Poultry meat and poultry meat products that are prescribed goods"@en-AU ;
    dct:isPartOf F2021L00310:15 ;
    dct:isReferencedBy F2021L00310: ;
    rdfs:comment "2 1  Poultry meat and poultry meat products that are prescribed goods - Abrievated Graph Key: I16"@en-AU ;
    skos:definition "2 1  Poultry meat and poultry meat products that are prescribed goods"@en-AU ;
    skos:narrower F2021L00310:15 ;
    skos:prefLabel "Item I16"@en-AU ;
    dcat:accessURL <https://www.legislation.gov.au/F2021L00310/2023-08-04/2023-08-04/text/1/epub/OEBPS/document_1/document_1.html#_Toc145601342> ;
    dcat:landingPage "https://www.legislation.gov.au/F2021L00310/2023-08-04/2023-08-04/text/1/epub/OEBPS/document_1/document_1.html#_Toc145601342"^^xsd:anyURI ;
    dcat:theme legcons:Item .

F2021L00310:161 a legcons:Item,
        owl:Class,
        dcat:Resource ;
    rdfs:label "Item - I161 8 8  Purpose of this Division"@en-AU ;
    dct:isPartOf F2021L00310:160 ;
    dct:isReferencedBy F2021L00310: ;
    rdfs:comment "8 8  Purpose of this Division - Abrievated Graph Key: I161"@en-AU ;
    skos:definition "8 8  Purpose of this Division"@en-AU ;
    skos:narrower F2021L00310:160 ;
    skos:prefLabel "Item I161"@en-AU ;
    dcat:accessURL <https://www.legislation.gov.au/F2021L00310/2023-08-04/2023-08-04/text/1/epub/OEBPS/document_1/document_1.html#_Toc145601487> ;
    dcat:landingPage "https://www.legislation.gov.au/F2021L00310/2023-08-04/2023-08-04/text/1/epub/OEBPS/document_1/document_1.html#_Toc145601487"^^xsd:anyURI ;
    dcat:theme legcons:Item .

F2021L00310:162 a legcons:Item,
        owl:Class,
        dcat:Resource ;
    rdfs:label "Item - I162 8 9  Tolerances for dimensions of official marks"@en-AU ;
    dct:isPartOf F2021L00310:160 ;
    dct:isReferencedBy F2021L00310: ;
    rdfs:comment "8 9  Tolerances for dimensions of official marks - Abrievated Graph Key: I162"@en-AU ;
    skos:definition "8 9  Tolerances for dimensions of official marks"@en-AU ;
    skos:narrower F2021L00310:160 ;
    skos:prefLabel "Item I162"@en-AU ;
    dcat:accessURL <https://www.legislation.gov.au/F2021L00310/2023-08-04/2023-08-04/text/1/epub/OEBPS/document_1/document_1.html#_Toc145601488> ;
    dcat:landingPage "https://www.legislation.gov.au/F2021L00310/2023-08-04/2023-08-04/text/1/epub/OEBPS/document_1/document_1.html#_Toc145601488"^^xsd:anyURI ;
    dcat:theme legcons:Item .

F2021L00310:163 a legcons:Item,
        owl:Class,
        dcat:Resource ;
    rdfs:label "Item - I163 8 10  Official markAustralia Inspected"@en-AU ;
    dct:isPartOf F2021L00310:160 ;
    dct:isReferencedBy F2021L00310: ;
    rdfs:comment "8 10  Official markAustralia Inspected - Abrievated Graph Key: I163"@en-AU ;
    skos:definition "8 10  Official markAustralia Inspected"@en-AU ;
    skos:narrower F2021L00310:160 ;
    skos:prefLabel "Item I163"@en-AU ;
    dcat:accessURL <https://www.legislation.gov.au/F2021L00310/2023-08-04/2023-08-04/text/1/epub/OEBPS/document_1/document_1.html#_Toc145601489> ;
    dcat:landingPage "https://www.legislation.gov.au/F2021L00310/2023-08-04/2023-08-04/text/1/epub/OEBPS/document_1/document_1.html#_Toc145601489"^^xsd:anyURI ;
    dcat:theme legcons:Item .

F2021L00310:164 a legcons:Item,
        owl:Class,
        dcat:Resource ;
    rdfs:label "Item - I164 8 11  Official markforeign country identification"@en-AU ;
    dct:isPartOf F2021L00310:160 ;
    dct:isReferencedBy F2021L00310: ;
    rdfs:comment "8 11  Official markforeign country identification - Abrievated Graph Key: I164"@en-AU ;
    skos:definition "8 11  Official markforeign country identification"@en-AU ;
    skos:narrower F2021L00310:160 ;
    skos:prefLabel "Item I164"@en-AU ;
    dcat:accessURL <https://www.legislation.gov.au/F2021L00310/2023-08-04/2023-08-04/text/1/epub/OEBPS/document_1/document_1.html#_Toc145601490> ;
    dcat:landingPage "https://www.legislation.gov.au/F2021L00310/2023-08-04/2023-08-04/text/1/epub/OEBPS/document_1/document_1.html#_Toc145601490"^^xsd:anyURI ;
    dcat:theme legcons:Item .

F2021L00310:165 a legcons:Item,
        owl:Class,
        dcat:Resource ;
    rdfs:label "Item - I165 8 12  Official marktamper indicative metal strap seal"@en-AU ;
    dct:isPartOf F2021L00310:160 ;
    dct:isReferencedBy F2021L00310: ;
    rdfs:comment "8 12  Official marktamper indicative metal strap seal - Abrievated Graph Key: I165"@en-AU ;
    skos:definition "8 12  Official marktamper indicative metal strap seal"@en-AU ;
    skos:narrower F2021L00310:160 ;
    skos:prefLabel "Item I165"@en-AU ;
    dcat:accessURL <https://www.legislation.gov.au/F2021L00310/2023-08-04/2023-08-04/text/1/epub/OEBPS/document_1/document_1.html#_Toc145601491> ;
    dcat:landingPage "https://www.legislation.gov.au/F2021L00310/2023-08-04/2023-08-04/text/1/epub/OEBPS/document_1/document_1.html#_Toc145601491"^^xsd:anyURI ;
    dcat:theme legcons:Item .

F2021L00310:166 a legcons:Item,
        owl:Class,
        dcat:Resource ;
    rdfs:label "Item - I166 8 13  Official markbolt seal"@en-AU ;
    dct:isPartOf F2021L00310:160 ;
    dct:isReferencedBy F2021L00310: ;
    rdfs:comment "8 13  Official markbolt seal - Abrievated Graph Key: I166"@en-AU ;
    skos:definition "8 13  Official markbolt seal"@en-AU ;
    skos:narrower F2021L00310:160 ;
    skos:prefLabel "Item I166"@en-AU ;
    dcat:accessURL <https://www.legislation.gov.au/F2021L00310/2023-08-04/2023-08-04/text/1/epub/OEBPS/document_1/document_1.html#_Toc145601492> ;
    dcat:landingPage "https://www.legislation.gov.au/F2021L00310/2023-08-04/2023-08-04/text/1/epub/OEBPS/document_1/document_1.html#_Toc145601492"^^xsd:anyURI ;
    dcat:theme legcons:Item .

F2021L00310:167 a legcons:Item,
        owl:Class,
        dcat:Resource ;
    rdfs:label "Item - I167 8 14  Official markAustralia Approved"@en-AU ;
    dct:isPartOf F2021L00310:160 ;
    dct:isReferencedBy F2021L00310: ;
    rdfs:comment "8 14  Official markAustralia Approved - Abrievated Graph Key: I167"@en-AU ;
    skos:definition "8 14  Official markAustralia Approved"@en-AU ;
    skos:narrower F2021L00310:160 ;
    skos:prefLabel "Item I167"@en-AU ;
    dcat:accessURL <https://www.legislation.gov.au/F2021L00310/2023-08-04/2023-08-04/text/1/epub/OEBPS/document_1/document_1.html#_Toc145601493> ;
    dcat:landingPage "https://www.legislation.gov.au/F2021L00310/2023-08-04/2023-08-04/text/1/epub/OEBPS/document_1/document_1.html#_Toc145601493"^^xsd:anyURI ;
    dcat:theme legcons:Item .

F2021L00310:168 a legcons:Item,
        owl:Class,
        dcat:Resource ;
    rdfs:label "Item - I168 8 15  Official markcarton seal"@en-AU ;
    dct:isPartOf F2021L00310:160 ;
    dct:isReferencedBy F2021L00310: ;
    rdfs:comment "8 15  Official markcarton seal - Abrievated Graph Key: I168"@en-AU ;
    skos:definition "8 15  Official markcarton seal"@en-AU ;
    skos:narrower F2021L00310:160 ;
    skos:prefLabel "Item I168"@en-AU ;
    dcat:accessURL <https://www.legislation.gov.au/F2021L00310/2023-08-04/2023-08-04/text/1/epub/OEBPS/document_1/document_1.html#_Toc145601494> ;
    dcat:landingPage "https://www.legislation.gov.au/F2021L00310/2023-08-04/2023-08-04/text/1/epub/OEBPS/document_1/document_1.html#_Toc145601494"^^xsd:anyURI ;
    dcat:theme legcons:Item .

F2021L00310:169 a legcons:Item,
        owl:Class,
        dcat:Resource ;
    rdfs:label "Item - I169 8 16  Official markpoultry meat or poultry meat products opened for assessment and resealed"@en-AU ;
    dct:isPartOf F2021L00310:160 ;
    dct:isReferencedBy F2021L00310: ;
    rdfs:comment "8 16  Official markpoultry meat or poultry meat products opened for assessment and resealed - Abrievated Graph Key: I169"@en-AU ;
    skos:definition "8 16  Official markpoultry meat or poultry meat products opened for assessment and resealed"@en-AU ;
    skos:narrower F2021L00310:160 ;
    skos:prefLabel "Item I169"@en-AU ;
    dcat:accessURL <https://www.legislation.gov.au/F2021L00310/2023-08-04/2023-08-04/text/1/epub/OEBPS/document_1/document_1.html#_Toc145601495> ;
    dcat:landingPage "https://www.legislation.gov.au/F2021L00310/2023-08-04/2023-08-04/text/1/epub/OEBPS/document_1/document_1.html#_Toc145601495"^^xsd:anyURI ;
    dcat:theme legcons:Item .

F2021L00310:17 a legcons:Item,
        owl:Class,
        dcat:Resource ;
    rdfs:label "Item - I17 2 2  Poultry meat and poultry meat products that are taken not to be prescribed goods"@en-AU ;
    dct:isPartOf F2021L00310:15 ;
    dct:isReferencedBy F2021L00310: ;
    rdfs:comment "2 2  Poultry meat and poultry meat products that are taken not to be prescribed goods - Abrievated Graph Key: I17"@en-AU ;
    skos:definition "2 2  Poultry meat and poultry meat products that are taken not to be prescribed goods"@en-AU ;
    skos:narrower F2021L00310:15 ;
    skos:prefLabel "Item I17"@en-AU ;
    dcat:accessURL <https://www.legislation.gov.au/F2021L00310/2023-08-04/2023-08-04/text/1/epub/OEBPS/document_1/document_1.html#_Toc145601343> ;
    dcat:landingPage "https://www.legislation.gov.au/F2021L00310/2023-08-04/2023-08-04/text/1/epub/OEBPS/document_1/document_1.html#_Toc145601343"^^xsd:anyURI ;
    dcat:theme legcons:Item .

F2021L00310:170 a legcons:Item,
        owl:Class,
        dcat:Resource ;
    rdfs:label "Item - I170 8 17  Official markAustralian Government"@en-AU ;
    dct:isPartOf F2021L00310:160 ;
    dct:isReferencedBy F2021L00310: ;
    rdfs:comment "8 17  Official markAustralian Government - Abrievated Graph Key: I170"@en-AU ;
    skos:definition "8 17  Official markAustralian Government"@en-AU ;
    skos:narrower F2021L00310:160 ;
    skos:prefLabel "Item I170"@en-AU ;
    dcat:accessURL <https://www.legislation.gov.au/F2021L00310/2023-08-04/2023-08-04/text/1/epub/OEBPS/document_1/document_1.html#_Toc145601496> ;
    dcat:landingPage "https://www.legislation.gov.au/F2021L00310/2023-08-04/2023-08-04/text/1/epub/OEBPS/document_1/document_1.html#_Toc145601496"^^xsd:anyURI ;
    dcat:theme legcons:Item .

F2021L00310:172 a legcons:Item,
        owl:Class,
        dcat:Resource ;
    rdfs:label "Item - I172 8 18  Purpose and application of this Division"@en-AU ;
    dct:isPartOf F2021L00310:171 ;
    dct:isReferencedBy F2021L00310: ;
    rdfs:comment "8 18  Purpose and application of this Division - Abrievated Graph Key: I172"@en-AU ;
    skos:definition "8 18  Purpose and application of this Division"@en-AU ;
    skos:narrower F2021L00310:171 ;
    skos:prefLabel "Item I172"@en-AU ;
    dcat:accessURL <https://www.legislation.gov.au/F2021L00310/2023-08-04/2023-08-04/text/1/epub/OEBPS/document_1/document_1.html#_Toc145601498> ;
    dcat:landingPage "https://www.legislation.gov.au/F2021L00310/2023-08-04/2023-08-04/text/1/epub/OEBPS/document_1/document_1.html#_Toc145601498"^^xsd:anyURI ;
    dcat:theme legcons:Item .

F2021L00310:173 a legcons:Item,
        owl:Class,
        dcat:Resource ;
    rdfs:label "Item - I173 8 19  Interpretation"@en-AU ;
    dct:isPartOf F2021L00310:171 ;
    dct:isReferencedBy F2021L00310: ;
    rdfs:comment "8 19  Interpretation - Abrievated Graph Key: I173"@en-AU ;
    skos:definition "8 19  Interpretation"@en-AU ;
    skos:narrower F2021L00310:171 ;
    skos:prefLabel "Item I173"@en-AU ;
    dcat:accessURL <https://www.legislation.gov.au/F2021L00310/2023-08-04/2023-08-04/text/1/epub/OEBPS/document_1/document_1.html#_Toc145601499> ;
    dcat:landingPage "https://www.legislation.gov.au/F2021L00310/2023-08-04/2023-08-04/text/1/epub/OEBPS/document_1/document_1.html#_Toc145601499"^^xsd:anyURI ;
    dcat:theme legcons:Item .

F2021L00310:174 a legcons:Item,
        owl:Class,
        dcat:Resource ;
    rdfs:label "Item - I174 8 20  Persons who may manufacture or supply official marks for poultry meat or poultry meat products"@en-AU ;
    dct:isPartOf F2021L00310:171 ;
    dct:isReferencedBy F2021L00310: ;
    rdfs:comment "8 20  Persons who may manufacture or supply official marks for poultry meat or poultry meat products - Abrievated Graph Key: I174"@en-AU ;
    skos:definition "8 20  Persons who may manufacture or supply official marks for poultry meat or poultry meat products"@en-AU ;
    skos:narrower F2021L00310:171 ;
    skos:prefLabel "Item I174"@en-AU ;
    dcat:accessURL <https://www.legislation.gov.au/F2021L00310/2023-08-04/2023-08-04/text/1/epub/OEBPS/document_1/document_1.html#_Toc145601500> ;
    dcat:landingPage "https://www.legislation.gov.au/F2021L00310/2023-08-04/2023-08-04/text/1/epub/OEBPS/document_1/document_1.html#_Toc145601500"^^xsd:anyURI ;
    dcat:theme legcons:Item .

F2021L00310:175 a legcons:Item,
        owl:Class,
        dcat:Resource ;
    rdfs:label "Item - I175 8 21  Persons who may possess official marks that have not been applied to poultry meat or poultry meat products"@en-AU ;
    dct:isPartOf F2021L00310:171 ;
    dct:isReferencedBy F2021L00310: ;
    rdfs:comment "8 21  Persons who may possess official marks that have not been applied to poultry meat or poultry meat products - Abrievated Graph Key: I175"@en-AU ;
    skos:definition "8 21  Persons who may possess official marks that have not been applied to poultry meat or poultry meat products"@en-AU ;
    skos:narrower F2021L00310:171 ;
    skos:prefLabel "Item I175"@en-AU ;
    dcat:accessURL <https://www.legislation.gov.au/F2021L00310/2023-08-04/2023-08-04/text/1/epub/OEBPS/document_1/document_1.html#_Toc145601501> ;
    dcat:landingPage "https://www.legislation.gov.au/F2021L00310/2023-08-04/2023-08-04/text/1/epub/OEBPS/document_1/document_1.html#_Toc145601501"^^xsd:anyURI ;
    dcat:theme legcons:Item .

F2021L00310:176 a legcons:Item,
        owl:Class,
        dcat:Resource ;
    rdfs:label "Item - I176 8 22  Persons who may apply official marks to poultry meat or poultry meat products etc"@en-AU ;
    dct:isPartOf F2021L00310:171 ;
    dct:isReferencedBy F2021L00310: ;
    rdfs:comment "8 22  Persons who may apply official marks to poultry meat or poultry meat products etc - Abrievated Graph Key: I176"@en-AU ;
    skos:definition "8 22  Persons who may apply official marks to poultry meat or poultry meat products etc"@en-AU ;
    skos:narrower F2021L00310:171 ;
    skos:prefLabel "Item I176"@en-AU ;
    dcat:accessURL <https://www.legislation.gov.au/F2021L00310/2023-08-04/2023-08-04/text/1/epub/OEBPS/document_1/document_1.html#_Toc145601502> ;
    dcat:landingPage "https://www.legislation.gov.au/F2021L00310/2023-08-04/2023-08-04/text/1/epub/OEBPS/document_1/document_1.html#_Toc145601502"^^xsd:anyURI ;
    dcat:theme legcons:Item .

F2021L00310:177 a legcons:Item,
        owl:Class,
        dcat:Resource ;
    rdfs:label "Item - I177 8 23  Circumstances in which official mark must not be applied to poultry meat or poultry meat products"@en-AU ;
    dct:isPartOf F2021L00310:171 ;
    dct:isReferencedBy F2021L00310: ;
    rdfs:comment "8 23  Circumstances in which official mark must not be applied to poultry meat or poultry meat products - Abrievated Graph Key: I177"@en-AU ;
    skos:definition "8 23  Circumstances in which official mark must not be applied to poultry meat or poultry meat products"@en-AU ;
    skos:narrower F2021L00310:171 ;
    skos:prefLabel "Item I177"@en-AU ;
    dcat:accessURL <https://www.legislation.gov.au/F2021L00310/2023-08-04/2023-08-04/text/1/epub/OEBPS/document_1/document_1.html#_Toc145601503> ;
    dcat:landingPage "https://www.legislation.gov.au/F2021L00310/2023-08-04/2023-08-04/text/1/epub/OEBPS/document_1/document_1.html#_Toc145601503"^^xsd:anyURI ;
    dcat:theme legcons:Item .

F2021L00310:178 a legcons:Item,
        owl:Class,
        dcat:Resource ;
    rdfs:label "Item - I178 8 24  Alteration of and interference with official marks"@en-AU ;
    dct:isPartOf F2021L00310:171 ;
    dct:isReferencedBy F2021L00310: ;
    rdfs:comment "8 24  Alteration of and interference with official marks - Abrievated Graph Key: I178"@en-AU ;
    skos:definition "8 24  Alteration of and interference with official marks"@en-AU ;
    skos:narrower F2021L00310:171 ;
    skos:prefLabel "Item I178"@en-AU ;
    dcat:accessURL <https://www.legislation.gov.au/F2021L00310/2023-08-04/2023-08-04/text/1/epub/OEBPS/document_1/document_1.html#_Toc145601504> ;
    dcat:landingPage "https://www.legislation.gov.au/F2021L00310/2023-08-04/2023-08-04/text/1/epub/OEBPS/document_1/document_1.html#_Toc145601504"^^xsd:anyURI ;
    dcat:theme legcons:Item .

F2021L00310:179 a legcons:Item,
        owl:Class,
        dcat:Resource ;
    rdfs:label "Item - I179 8 25  Official marks must be legible and securely attached"@en-AU ;
    dct:isPartOf F2021L00310:171 ;
    dct:isReferencedBy F2021L00310: ;
    rdfs:comment "8 25  Official marks must be legible and securely attached - Abrievated Graph Key: I179"@en-AU ;
    skos:definition "8 25  Official marks must be legible and securely attached"@en-AU ;
    skos:narrower F2021L00310:171 ;
    skos:prefLabel "Item I179"@en-AU ;
    dcat:accessURL <https://www.legislation.gov.au/F2021L00310/2023-08-04/2023-08-04/text/1/epub/OEBPS/document_1/document_1.html#_Toc145601505> ;
    dcat:landingPage "https://www.legislation.gov.au/F2021L00310/2023-08-04/2023-08-04/text/1/epub/OEBPS/document_1/document_1.html#_Toc145601505"^^xsd:anyURI ;
    dcat:theme legcons:Item .

F2021L00310:180 a legcons:Item,
        owl:Class,
        dcat:Resource ;
    rdfs:label "Item - I180 8 26  Security of official marks"@en-AU ;
    dct:isPartOf F2021L00310:171 ;
    dct:isReferencedBy F2021L00310: ;
    rdfs:comment "8 26  Security of official marks - Abrievated Graph Key: I180"@en-AU ;
    skos:definition "8 26  Security of official marks"@en-AU ;
    skos:narrower F2021L00310:171 ;
    skos:prefLabel "Item I180"@en-AU ;
    dcat:accessURL <https://www.legislation.gov.au/F2021L00310/2023-08-04/2023-08-04/text/1/epub/OEBPS/document_1/document_1.html#_Toc145601506> ;
    dcat:landingPage "https://www.legislation.gov.au/F2021L00310/2023-08-04/2023-08-04/text/1/epub/OEBPS/document_1/document_1.html#_Toc145601506"^^xsd:anyURI ;
    dcat:theme legcons:Item .

F2021L00310:181 a legcons:Item,
        owl:Class,
        dcat:Resource ;
    rdfs:label "Item - I181 8 27  Removal or defacement of official marks"@en-AU ;
    dct:isPartOf F2021L00310:171 ;
    dct:isReferencedBy F2021L00310: ;
    rdfs:comment "8 27  Removal or defacement of official marks - Abrievated Graph Key: I181"@en-AU ;
    skos:definition "8 27  Removal or defacement of official marks"@en-AU ;
    skos:narrower F2021L00310:171 ;
    skos:prefLabel "Item I181"@en-AU ;
    dcat:accessURL <https://www.legislation.gov.au/F2021L00310/2023-08-04/2023-08-04/text/1/epub/OEBPS/document_1/document_1.html#_Toc145601507> ;
    dcat:landingPage "https://www.legislation.gov.au/F2021L00310/2023-08-04/2023-08-04/text/1/epub/OEBPS/document_1/document_1.html#_Toc145601507"^^xsd:anyURI ;
    dcat:theme legcons:Item .

F2021L00310:182 a legcons:Item,
        owl:Class,
        dcat:Resource ;
    rdfs:label "Item - I182 8 28  Records of official marks manufactured or supplied"@en-AU ;
    dct:isPartOf F2021L00310:171 ;
    dct:isReferencedBy F2021L00310: ;
    rdfs:comment "8 28  Records of official marks manufactured or supplied - Abrievated Graph Key: I182"@en-AU ;
    skos:definition "8 28  Records of official marks manufactured or supplied"@en-AU ;
    skos:narrower F2021L00310:171 ;
    skos:prefLabel "Item I182"@en-AU ;
    dcat:accessURL <https://www.legislation.gov.au/F2021L00310/2023-08-04/2023-08-04/text/1/epub/OEBPS/document_1/document_1.html#_Toc145601508> ;
    dcat:landingPage "https://www.legislation.gov.au/F2021L00310/2023-08-04/2023-08-04/text/1/epub/OEBPS/document_1/document_1.html#_Toc145601508"^^xsd:anyURI ;
    dcat:theme legcons:Item .

F2021L00310:183 a legcons:Item,
        owl:Class,
        dcat:Resource ;
    rdfs:label "Item - I183 8 29  Records of official marks received applied removed defaced destroyed or returned"@en-AU ;
    dct:isPartOf F2021L00310:171 ;
    dct:isReferencedBy F2021L00310: ;
    rdfs:comment "8 29  Records of official marks received applied removed defaced destroyed or returned - Abrievated Graph Key: I183"@en-AU ;
    skos:definition "8 29  Records of official marks received applied removed defaced destroyed or returned"@en-AU ;
    skos:narrower F2021L00310:171 ;
    skos:prefLabel "Item I183"@en-AU ;
    dcat:accessURL <https://www.legislation.gov.au/F2021L00310/2023-08-04/2023-08-04/text/1/epub/OEBPS/document_1/document_1.html#_Toc145601509> ;
    dcat:landingPage "https://www.legislation.gov.au/F2021L00310/2023-08-04/2023-08-04/text/1/epub/OEBPS/document_1/document_1.html#_Toc145601509"^^xsd:anyURI ;
    dcat:theme legcons:Item .

F2021L00310:185 a legcons:Item,
        owl:Class,
        dcat:Resource ;
    rdfs:label "Item - I185 8 30  Purpose of this Division"@en-AU ;
    dct:isPartOf F2021L00310:184 ;
    dct:isReferencedBy F2021L00310: ;
    rdfs:comment "8 30  Purpose of this Division - Abrievated Graph Key: I185"@en-AU ;
    skos:definition "8 30  Purpose of this Division"@en-AU ;
    skos:narrower F2021L00310:184 ;
    skos:prefLabel "Item I185"@en-AU ;
    dcat:accessURL <https://www.legislation.gov.au/F2021L00310/2023-08-04/2023-08-04/text/1/epub/OEBPS/document_1/document_1.html#_Toc145601511> ;
    dcat:landingPage "https://www.legislation.gov.au/F2021L00310/2023-08-04/2023-08-04/text/1/epub/OEBPS/document_1/document_1.html#_Toc145601511"^^xsd:anyURI ;
    dcat:theme legcons:Item .

F2021L00310:186 a legcons:Item,
        owl:Class,
        dcat:Resource ;
    rdfs:label "Item - I186 8 31  Circumstances in which a mark resembles an official mark"@en-AU ;
    dct:isPartOf F2021L00310:184 ;
    dct:isReferencedBy F2021L00310: ;
    rdfs:comment "8 31  Circumstances in which a mark resembles an official mark - Abrievated Graph Key: I186"@en-AU ;
    skos:definition "8 31  Circumstances in which a mark resembles an official mark"@en-AU ;
    skos:narrower F2021L00310:184 ;
    skos:prefLabel "Item I186"@en-AU ;
    dcat:accessURL <https://www.legislation.gov.au/F2021L00310/2023-08-04/2023-08-04/text/1/epub/OEBPS/document_1/document_1.html#_Toc145601512> ;
    dcat:landingPage "https://www.legislation.gov.au/F2021L00310/2023-08-04/2023-08-04/text/1/epub/OEBPS/document_1/document_1.html#_Toc145601512"^^xsd:anyURI ;
    dcat:theme legcons:Item .

F2021L00310:187 a legcons:Item,
        owl:Class,
        dcat:Resource ;
    rdfs:label "Item - I187 8 32  Persons who may apply a resemblance"@en-AU ;
    dct:isPartOf F2021L00310:184 ;
    dct:isReferencedBy F2021L00310: ;
    rdfs:comment "8 32  Persons who may apply a resemblance - Abrievated Graph Key: I187"@en-AU ;
    skos:definition "8 32  Persons who may apply a resemblance"@en-AU ;
    skos:narrower F2021L00310:184 ;
    skos:prefLabel "Item I187"@en-AU ;
    dcat:accessURL <https://www.legislation.gov.au/F2021L00310/2023-08-04/2023-08-04/text/1/epub/OEBPS/document_1/document_1.html#_Toc145601513> ;
    dcat:landingPage "https://www.legislation.gov.au/F2021L00310/2023-08-04/2023-08-04/text/1/epub/OEBPS/document_1/document_1.html#_Toc145601513"^^xsd:anyURI ;
    dcat:theme legcons:Item .

F2021L00310:189 a legcons:Item,
        owl:Class,
        dcat:Resource ;
    rdfs:label "Item - I189 8 33  Purpose of this Division"@en-AU ;
    dct:isPartOf F2021L00310:188 ;
    dct:isReferencedBy F2021L00310: ;
    rdfs:comment "8 33  Purpose of this Division - Abrievated Graph Key: I189"@en-AU ;
    skos:definition "8 33  Purpose of this Division"@en-AU ;
    skos:narrower F2021L00310:188 ;
    skos:prefLabel "Item I189"@en-AU ;
    dcat:accessURL <https://www.legislation.gov.au/F2021L00310/2023-08-04/2023-08-04/text/1/epub/OEBPS/document_1/document_1.html#_Toc145601515> ;
    dcat:landingPage "https://www.legislation.gov.au/F2021L00310/2023-08-04/2023-08-04/text/1/epub/OEBPS/document_1/document_1.html#_Toc145601515"^^xsd:anyURI ;
    dcat:theme legcons:Item .

F2021L00310:19 a legcons:Item,
        owl:Class,
        dcat:Resource ;
    rdfs:label "Item - I19 2 3  Purpose and application of this Division"@en-AU ;
    dct:isPartOf F2021L00310:18 ;
    dct:isReferencedBy F2021L00310: ;
    rdfs:comment "2 3  Purpose and application of this Division - Abrievated Graph Key: I19"@en-AU ;
    skos:definition "2 3  Purpose and application of this Division"@en-AU ;
    skos:narrower F2021L00310:18 ;
    skos:prefLabel "Item I19"@en-AU ;
    dcat:accessURL <https://www.legislation.gov.au/F2021L00310/2023-08-04/2023-08-04/text/1/epub/OEBPS/document_1/document_1.html#_Toc145601345> ;
    dcat:landingPage "https://www.legislation.gov.au/F2021L00310/2023-08-04/2023-08-04/text/1/epub/OEBPS/document_1/document_1.html#_Toc145601345"^^xsd:anyURI ;
    dcat:theme legcons:Item .

F2021L00310:190 a legcons:Item,
        owl:Class,
        dcat:Resource ;
    rdfs:label "Item - I190 8 34  Persons who may manufacture supply or possess official marking devices"@en-AU ;
    dct:isPartOf F2021L00310:188 ;
    dct:isReferencedBy F2021L00310: ;
    rdfs:comment "8 34  Persons who may manufacture supply or possess official marking devices - Abrievated Graph Key: I190"@en-AU ;
    skos:definition "8 34  Persons who may manufacture supply or possess official marking devices"@en-AU ;
    skos:narrower F2021L00310:188 ;
    skos:prefLabel "Item I190"@en-AU ;
    dcat:accessURL <https://www.legislation.gov.au/F2021L00310/2023-08-04/2023-08-04/text/1/epub/OEBPS/document_1/document_1.html#_Toc145601516> ;
    dcat:landingPage "https://www.legislation.gov.au/F2021L00310/2023-08-04/2023-08-04/text/1/epub/OEBPS/document_1/document_1.html#_Toc145601516"^^xsd:anyURI ;
    dcat:theme legcons:Item .

F2021L00310:191 a legcons:Item,
        owl:Class,
        dcat:Resource ;
    rdfs:label "Item - I191 8 35  Security of official marking devices"@en-AU ;
    dct:isPartOf F2021L00310:188 ;
    dct:isReferencedBy F2021L00310: ;
    rdfs:comment "8 35  Security of official marking devices - Abrievated Graph Key: I191"@en-AU ;
    skos:definition "8 35  Security of official marking devices"@en-AU ;
    skos:narrower F2021L00310:188 ;
    skos:prefLabel "Item I191"@en-AU ;
    dcat:accessURL <https://www.legislation.gov.au/F2021L00310/2023-08-04/2023-08-04/text/1/epub/OEBPS/document_1/document_1.html#_Toc145601517> ;
    dcat:landingPage "https://www.legislation.gov.au/F2021L00310/2023-08-04/2023-08-04/text/1/epub/OEBPS/document_1/document_1.html#_Toc145601517"^^xsd:anyURI ;
    dcat:theme legcons:Item .

F2021L00310:192 a legcons:Item,
        owl:Class,
        dcat:Resource ;
    rdfs:label "Item - I192 8 36  Damaged etc official marking devices"@en-AU ;
    dct:isPartOf F2021L00310:188 ;
    dct:isReferencedBy F2021L00310: ;
    rdfs:comment "8 36  Damaged etc official marking devices - Abrievated Graph Key: I192"@en-AU ;
    skos:definition "8 36  Damaged etc official marking devices"@en-AU ;
    skos:narrower F2021L00310:188 ;
    skos:prefLabel "Item I192"@en-AU ;
    dcat:accessURL <https://www.legislation.gov.au/F2021L00310/2023-08-04/2023-08-04/text/1/epub/OEBPS/document_1/document_1.html#_Toc145601518> ;
    dcat:landingPage "https://www.legislation.gov.au/F2021L00310/2023-08-04/2023-08-04/text/1/epub/OEBPS/document_1/document_1.html#_Toc145601518"^^xsd:anyURI ;
    dcat:theme legcons:Item .

F2021L00310:193 a legcons:Item,
        owl:Class,
        dcat:Resource ;
    rdfs:label "Item - I193 8 37  Records of official marking devices manufactured or supplied"@en-AU ;
    dct:isPartOf F2021L00310:188 ;
    dct:isReferencedBy F2021L00310: ;
    rdfs:comment "8 37  Records of official marking devices manufactured or supplied - Abrievated Graph Key: I193"@en-AU ;
    skos:definition "8 37  Records of official marking devices manufactured or supplied"@en-AU ;
    skos:narrower F2021L00310:188 ;
    skos:prefLabel "Item I193"@en-AU ;
    dcat:accessURL <https://www.legislation.gov.au/F2021L00310/2023-08-04/2023-08-04/text/1/epub/OEBPS/document_1/document_1.html#_Toc145601519> ;
    dcat:landingPage "https://www.legislation.gov.au/F2021L00310/2023-08-04/2023-08-04/text/1/epub/OEBPS/document_1/document_1.html#_Toc145601519"^^xsd:anyURI ;
    dcat:theme legcons:Item .

F2021L00310:194 a legcons:Item,
        owl:Class,
        dcat:Resource ;
    rdfs:label "Item - I194 8 38  Records of official marking devices received used damaged destroyed or returned"@en-AU ;
    dct:isPartOf F2021L00310:188 ;
    dct:isReferencedBy F2021L00310: ;
    rdfs:comment "8 38  Records of official marking devices received used damaged destroyed or returned - Abrievated Graph Key: I194"@en-AU ;
    skos:definition "8 38  Records of official marking devices received used damaged destroyed or returned"@en-AU ;
    skos:narrower F2021L00310:188 ;
    skos:prefLabel "Item I194"@en-AU ;
    dcat:accessURL <https://www.legislation.gov.au/F2021L00310/2023-08-04/2023-08-04/text/1/epub/OEBPS/document_1/document_1.html#_Toc145601520> ;
    dcat:landingPage "https://www.legislation.gov.au/F2021L00310/2023-08-04/2023-08-04/text/1/epub/OEBPS/document_1/document_1.html#_Toc145601520"^^xsd:anyURI ;
    dcat:theme legcons:Item .

F2021L00310:198 a legcons:Item,
        owl:Class,
        dcat:Resource ;
    rdfs:label "Item - I198 9 1  References to audit in this Part"@en-AU ;
    dct:isPartOf F2021L00310:197 ;
    dct:isReferencedBy F2021L00310: ;
    rdfs:comment "9 1  References to audit in this Part - Abrievated Graph Key: I198"@en-AU ;
    skos:definition "9 1  References to audit in this Part"@en-AU ;
    skos:narrower F2021L00310:197 ;
    skos:prefLabel "Item I198"@en-AU ;
    dcat:accessURL <https://www.legislation.gov.au/F2021L00310/2023-08-04/2023-08-04/text/1/epub/OEBPS/document_1/document_1.html#_Toc145601524> ;
    dcat:landingPage "https://www.legislation.gov.au/F2021L00310/2023-08-04/2023-08-04/text/1/epub/OEBPS/document_1/document_1.html#_Toc145601524"^^xsd:anyURI ;
    dcat:theme legcons:Item .

F2021L00310:2 a legcons:Part,
        owl:Class,
        dcat:Resource ;
    rdfs:label "Part - P2 Part 1 Preliminary"@en-AU ;
    dct:isPartOf F2021L00310:1 ;
    dct:isReferencedBy F2021L00310: ;
    rdfs:comment "Part 1 Preliminary - Abrievated Graph Key: P2"@en-AU ;
    skos:definition "Part 1 Preliminary"@en-AU ;
    skos:narrower F2021L00310:1 ;
    skos:prefLabel "Part P2"@en-AU ;
    dcat:accessURL <https://www.legislation.gov.au/F2021L00310/2023-08-04/2023-08-04/text/1/epub/OEBPS/document_1/document_1.html#_Toc145601328> ;
    dcat:landingPage "https://www.legislation.gov.au/F2021L00310/2023-08-04/2023-08-04/text/1/epub/OEBPS/document_1/document_1.html#_Toc145601328"^^xsd:anyURI ;
    dcat:theme legcons:Part .

F2021L00310:20 a legcons:Item,
        owl:Class,
        dcat:Resource ;
    rdfs:label "Item - I20 2 4  Export of prescribed poultry meat or poultry meat products is prohibited unless prescribed conditions are complied with"@en-AU ;
    dct:isPartOf F2021L00310:18 ;
    dct:isReferencedBy F2021L00310: ;
    rdfs:comment "2 4  Export of prescribed poultry meat or poultry meat products is prohibited unless prescribed conditions are complied with - Abrievated Graph Key: I20"@en-AU ;
    skos:definition "2 4  Export of prescribed poultry meat or poultry meat products is prohibited unless prescribed conditions are complied with"@en-AU ;
    skos:narrower F2021L00310:18 ;
    skos:prefLabel "Item I20"@en-AU ;
    dcat:accessURL <https://www.legislation.gov.au/F2021L00310/2023-08-04/2023-08-04/text/1/epub/OEBPS/document_1/document_1.html#_Toc145601346> ;
    dcat:landingPage "https://www.legislation.gov.au/F2021L00310/2023-08-04/2023-08-04/text/1/epub/OEBPS/document_1/document_1.html#_Toc145601346"^^xsd:anyURI ;
    dcat:theme legcons:Item .

F2021L00310:200 a legcons:Item,
        owl:Class,
        dcat:Resource ;
    rdfs:label "Item - I200 9 2  Purpose of this Division"@en-AU ;
    dct:isPartOf F2021L00310:199 ;
    dct:isReferencedBy F2021L00310: ;
    rdfs:comment "9 2  Purpose of this Division - Abrievated Graph Key: I200"@en-AU ;
    skos:definition "9 2  Purpose of this Division"@en-AU ;
    skos:narrower F2021L00310:199 ;
    skos:prefLabel "Item I200"@en-AU ;
    dcat:accessURL <https://www.legislation.gov.au/F2021L00310/2023-08-04/2023-08-04/text/1/epub/OEBPS/document_1/document_1.html#_Toc145601526> ;
    dcat:landingPage "https://www.legislation.gov.au/F2021L00310/2023-08-04/2023-08-04/text/1/epub/OEBPS/document_1/document_1.html#_Toc145601526"^^xsd:anyURI ;
    dcat:theme legcons:Item .

F2021L00310:201 a legcons:Item,
        owl:Class,
        dcat:Resource ;
    rdfs:label "Item - I201 9 3  Manner in which audit must be conducted"@en-AU ;
    dct:isPartOf F2021L00310:199 ;
    dct:isReferencedBy F2021L00310: ;
    rdfs:comment "9 3  Manner in which audit must be conducted - Abrievated Graph Key: I201"@en-AU ;
    skos:definition "9 3  Manner in which audit must be conducted"@en-AU ;
    skos:narrower F2021L00310:199 ;
    skos:prefLabel "Item I201"@en-AU ;
    dcat:accessURL <https://www.legislation.gov.au/F2021L00310/2023-08-04/2023-08-04/text/1/epub/OEBPS/document_1/document_1.html#_Toc145601527> ;
    dcat:landingPage "https://www.legislation.gov.au/F2021L00310/2023-08-04/2023-08-04/text/1/epub/OEBPS/document_1/document_1.html#_Toc145601527"^^xsd:anyURI ;
    dcat:theme legcons:Item .

F2021L00310:202 a legcons:Item,
        owl:Class,
        dcat:Resource ;
    rdfs:label "Item - I202 9 4  Notice of non compliance with requirements"@en-AU ;
    dct:isPartOf F2021L00310:199 ;
    dct:isReferencedBy F2021L00310: ;
    rdfs:comment "9 4  Notice of non compliance with requirements - Abrievated Graph Key: I202"@en-AU ;
    skos:definition "9 4  Notice of non compliance with requirements"@en-AU ;
    skos:narrower F2021L00310:199 ;
    skos:prefLabel "Item I202"@en-AU ;
    dcat:accessURL <https://www.legislation.gov.au/F2021L00310/2023-08-04/2023-08-04/text/1/epub/OEBPS/document_1/document_1.html#_Toc145601528> ;
    dcat:landingPage "https://www.legislation.gov.au/F2021L00310/2023-08-04/2023-08-04/text/1/epub/OEBPS/document_1/document_1.html#_Toc145601528"^^xsd:anyURI ;
    dcat:theme legcons:Item .

F2021L00310:203 a legcons:Item,
        owl:Class,
        dcat:Resource ;
    rdfs:label "Item - I203 9 5  Audit reports"@en-AU ;
    dct:isPartOf F2021L00310:199 ;
    dct:isReferencedBy F2021L00310: ;
    rdfs:comment "9 5  Audit reports - Abrievated Graph Key: I203"@en-AU ;
    skos:definition "9 5  Audit reports"@en-AU ;
    skos:narrower F2021L00310:199 ;
    skos:prefLabel "Item I203"@en-AU ;
    dcat:accessURL <https://www.legislation.gov.au/F2021L00310/2023-08-04/2023-08-04/text/1/epub/OEBPS/document_1/document_1.html#_Toc145601529> ;
    dcat:landingPage "https://www.legislation.gov.au/F2021L00310/2023-08-04/2023-08-04/text/1/epub/OEBPS/document_1/document_1.html#_Toc145601529"^^xsd:anyURI ;
    dcat:theme legcons:Item .

F2021L00310:205 a legcons:Item,
        owl:Class,
        dcat:Resource ;
    rdfs:label "Item - I205 9 6  Purpose of this Division"@en-AU ;
    dct:isPartOf F2021L00310:204 ;
    dct:isReferencedBy F2021L00310: ;
    rdfs:comment "9 6  Purpose of this Division - Abrievated Graph Key: I205"@en-AU ;
    skos:definition "9 6  Purpose of this Division"@en-AU ;
    skos:narrower F2021L00310:204 ;
    skos:prefLabel "Item I205"@en-AU ;
    dcat:accessURL <https://www.legislation.gov.au/F2021L00310/2023-08-04/2023-08-04/text/1/epub/OEBPS/document_1/document_1.html#_Toc145601531> ;
    dcat:landingPage "https://www.legislation.gov.au/F2021L00310/2023-08-04/2023-08-04/text/1/epub/OEBPS/document_1/document_1.html#_Toc145601531"^^xsd:anyURI ;
    dcat:theme legcons:Item .

F2021L00310:206 a legcons:Item,
        owl:Class,
        dcat:Resource ;
    rdfs:label "Item - I206 9 7  Application for approval"@en-AU ;
    dct:isPartOf F2021L00310:204 ;
    dct:isReferencedBy F2021L00310: ;
    rdfs:comment "9 7  Application for approval - Abrievated Graph Key: I206"@en-AU ;
    skos:definition "9 7  Application for approval"@en-AU ;
    skos:narrower F2021L00310:204 ;
    skos:prefLabel "Item I206"@en-AU ;
    dcat:accessURL <https://www.legislation.gov.au/F2021L00310/2023-08-04/2023-08-04/text/1/epub/OEBPS/document_1/document_1.html#_Toc145601532> ;
    dcat:landingPage "https://www.legislation.gov.au/F2021L00310/2023-08-04/2023-08-04/text/1/epub/OEBPS/document_1/document_1.html#_Toc145601532"^^xsd:anyURI ;
    dcat:theme legcons:Item .

F2021L00310:207 a legcons:Item,
        owl:Class,
        dcat:Resource ;
    rdfs:label "Item - I207 9 8  Secretary must decide whether to approve applicant to conduct audits"@en-AU ;
    dct:isPartOf F2021L00310:204 ;
    dct:isReferencedBy F2021L00310: ;
    rdfs:comment "9 8  Secretary must decide whether to approve applicant to conduct audits - Abrievated Graph Key: I207"@en-AU ;
    skos:definition "9 8  Secretary must decide whether to approve applicant to conduct audits"@en-AU ;
    skos:narrower F2021L00310:204 ;
    skos:prefLabel "Item I207"@en-AU ;
    dcat:accessURL <https://www.legislation.gov.au/F2021L00310/2023-08-04/2023-08-04/text/1/epub/OEBPS/document_1/document_1.html#_Toc145601533> ;
    dcat:landingPage "https://www.legislation.gov.au/F2021L00310/2023-08-04/2023-08-04/text/1/epub/OEBPS/document_1/document_1.html#_Toc145601533"^^xsd:anyURI ;
    dcat:theme legcons:Item .

F2021L00310:208 a legcons:Item,
        owl:Class,
        dcat:Resource ;
    rdfs:label "Item - I208 9 9  Dealing with applications"@en-AU ;
    dct:isPartOf F2021L00310:204 ;
    dct:isReferencedBy F2021L00310: ;
    rdfs:comment "9 9  Dealing with applications - Abrievated Graph Key: I208"@en-AU ;
    skos:definition "9 9  Dealing with applications"@en-AU ;
    skos:narrower F2021L00310:204 ;
    skos:prefLabel "Item I208"@en-AU ;
    dcat:accessURL <https://www.legislation.gov.au/F2021L00310/2023-08-04/2023-08-04/text/1/epub/OEBPS/document_1/document_1.html#_Toc145601534> ;
    dcat:landingPage "https://www.legislation.gov.au/F2021L00310/2023-08-04/2023-08-04/text/1/epub/OEBPS/document_1/document_1.html#_Toc145601534"^^xsd:anyURI ;
    dcat:theme legcons:Item .

F2021L00310:209 a legcons:Item,
        owl:Class,
        dcat:Resource ;
    rdfs:label "Item - I209 9 10  Conditions of approval"@en-AU ;
    dct:isPartOf F2021L00310:204 ;
    dct:isReferencedBy F2021L00310: ;
    rdfs:comment "9 10  Conditions of approval - Abrievated Graph Key: I209"@en-AU ;
    skos:definition "9 10  Conditions of approval"@en-AU ;
    skos:narrower F2021L00310:204 ;
    skos:prefLabel "Item I209"@en-AU ;
    dcat:accessURL <https://www.legislation.gov.au/F2021L00310/2023-08-04/2023-08-04/text/1/epub/OEBPS/document_1/document_1.html#_Toc145601535> ;
    dcat:landingPage "https://www.legislation.gov.au/F2021L00310/2023-08-04/2023-08-04/text/1/epub/OEBPS/document_1/document_1.html#_Toc145601535"^^xsd:anyURI ;
    dcat:theme legcons:Item .

F2021L00310:210 a legcons:Item,
        owl:Class,
        dcat:Resource ;
    rdfs:label "Item - I210 9 11  Notice of decision"@en-AU ;
    dct:isPartOf F2021L00310:204 ;
    dct:isReferencedBy F2021L00310: ;
    rdfs:comment "9 11  Notice of decision - Abrievated Graph Key: I210"@en-AU ;
    skos:definition "9 11  Notice of decision"@en-AU ;
    skos:narrower F2021L00310:204 ;
    skos:prefLabel "Item I210"@en-AU ;
    dcat:accessURL <https://www.legislation.gov.au/F2021L00310/2023-08-04/2023-08-04/text/1/epub/OEBPS/document_1/document_1.html#_Toc145601536> ;
    dcat:landingPage "https://www.legislation.gov.au/F2021L00310/2023-08-04/2023-08-04/text/1/epub/OEBPS/document_1/document_1.html#_Toc145601536"^^xsd:anyURI ;
    dcat:theme legcons:Item .

F2021L00310:211 a legcons:Item,
        owl:Class,
        dcat:Resource ;
    rdfs:label "Item - I211 9 12  Period of effect of approval"@en-AU ;
    dct:isPartOf F2021L00310:204 ;
    dct:isReferencedBy F2021L00310: ;
    rdfs:comment "9 12  Period of effect of approval - Abrievated Graph Key: I211"@en-AU ;
    skos:definition "9 12  Period of effect of approval"@en-AU ;
    skos:narrower F2021L00310:204 ;
    skos:prefLabel "Item I211"@en-AU ;
    dcat:accessURL <https://www.legislation.gov.au/F2021L00310/2023-08-04/2023-08-04/text/1/epub/OEBPS/document_1/document_1.html#_Toc145601537> ;
    dcat:landingPage "https://www.legislation.gov.au/F2021L00310/2023-08-04/2023-08-04/text/1/epub/OEBPS/document_1/document_1.html#_Toc145601537"^^xsd:anyURI ;
    dcat:theme legcons:Item .

F2021L00310:212 a legcons:Item,
        owl:Class,
        dcat:Resource ;
    rdfs:label "Item - I212 9 13  Imposing or varying conditions of approval"@en-AU ;
    dct:isPartOf F2021L00310:204 ;
    dct:isReferencedBy F2021L00310: ;
    rdfs:comment "9 13  Imposing or varying conditions of approval - Abrievated Graph Key: I212"@en-AU ;
    skos:definition "9 13  Imposing or varying conditions of approval"@en-AU ;
    skos:narrower F2021L00310:204 ;
    skos:prefLabel "Item I212"@en-AU ;
    dcat:accessURL <https://www.legislation.gov.au/F2021L00310/2023-08-04/2023-08-04/text/1/epub/OEBPS/document_1/document_1.html#_Toc145601538> ;
    dcat:landingPage "https://www.legislation.gov.au/F2021L00310/2023-08-04/2023-08-04/text/1/epub/OEBPS/document_1/document_1.html#_Toc145601538"^^xsd:anyURI ;
    dcat:theme legcons:Item .

F2021L00310:213 a legcons:Item,
        owl:Class,
        dcat:Resource ;
    rdfs:label "Item - I213 9 14  Revocation of approval"@en-AU ;
    dct:isPartOf F2021L00310:204 ;
    dct:isReferencedBy F2021L00310: ;
    rdfs:comment "9 14  Revocation of approval - Abrievated Graph Key: I213"@en-AU ;
    skos:definition "9 14  Revocation of approval"@en-AU ;
    skos:narrower F2021L00310:204 ;
    skos:prefLabel "Item I213"@en-AU ;
    dcat:accessURL <https://www.legislation.gov.au/F2021L00310/2023-08-04/2023-08-04/text/1/epub/OEBPS/document_1/document_1.html#_Toc145601539> ;
    dcat:landingPage "https://www.legislation.gov.au/F2021L00310/2023-08-04/2023-08-04/text/1/epub/OEBPS/document_1/document_1.html#_Toc145601539"^^xsd:anyURI ;
    dcat:theme legcons:Item .

F2021L00310:214 a legcons:Item,
        owl:Class,
        dcat:Resource ;
    rdfs:label "Item - I214 9 15  Register of approved auditors"@en-AU ;
    dct:isPartOf F2021L00310:204 ;
    dct:isReferencedBy F2021L00310: ;
    rdfs:comment "9 15  Register of approved auditors - Abrievated Graph Key: I214"@en-AU ;
    skos:definition "9 15  Register of approved auditors"@en-AU ;
    skos:narrower F2021L00310:204 ;
    skos:prefLabel "Item I214"@en-AU ;
    dcat:accessURL <https://www.legislation.gov.au/F2021L00310/2023-08-04/2023-08-04/text/1/epub/OEBPS/document_1/document_1.html#_Toc145601540> ;
    dcat:landingPage "https://www.legislation.gov.au/F2021L00310/2023-08-04/2023-08-04/text/1/epub/OEBPS/document_1/document_1.html#_Toc145601540"^^xsd:anyURI ;
    dcat:theme legcons:Item .

F2021L00310:215 a legcons:Item,
        owl:Class,
        dcat:Resource ;
    rdfs:label "Item - I215 9 16  Fit and proper person test"@en-AU ;
    dct:isPartOf F2021L00310:204 ;
    dct:isReferencedBy F2021L00310: ;
    rdfs:comment "9 16  Fit and proper person test - Abrievated Graph Key: I215"@en-AU ;
    skos:definition "9 16  Fit and proper person test"@en-AU ;
    skos:narrower F2021L00310:204 ;
    skos:prefLabel "Item I215"@en-AU ;
    dcat:accessURL <https://www.legislation.gov.au/F2021L00310/2023-08-04/2023-08-04/text/1/epub/OEBPS/document_1/document_1.html#_Toc145601541> ;
    dcat:landingPage "https://www.legislation.gov.au/F2021L00310/2023-08-04/2023-08-04/text/1/epub/OEBPS/document_1/document_1.html#_Toc145601541"^^xsd:anyURI ;
    dcat:theme legcons:Item .

F2021L00310:217 a legcons:Item,
        owl:Class,
        dcat:Resource ;
    rdfs:label "Item - I217 9 17  Circumstances in which assessment may be required or permitted"@en-AU ;
    dct:isPartOf F2021L00310:216 ;
    dct:isReferencedBy F2021L00310: ;
    rdfs:comment "9 17  Circumstances in which assessment may be required or permitted - Abrievated Graph Key: I217"@en-AU ;
    skos:definition "9 17  Circumstances in which assessment may be required or permitted"@en-AU ;
    skos:narrower F2021L00310:216 ;
    skos:prefLabel "Item I217"@en-AU ;
    dcat:accessURL <https://www.legislation.gov.au/F2021L00310/2023-08-04/2023-08-04/text/1/epub/OEBPS/document_1/document_1.html#_Toc145601543> ;
    dcat:landingPage "https://www.legislation.gov.au/F2021L00310/2023-08-04/2023-08-04/text/1/epub/OEBPS/document_1/document_1.html#_Toc145601543"^^xsd:anyURI ;
    dcat:theme legcons:Item .

F2021L00310:219 a legcons:Item,
        owl:Class,
        dcat:Resource ;
    rdfs:label "Item - I219 9 18  Decisions that may be made by operation of computer program"@en-AU ;
    dct:isPartOf F2021L00310:218 ;
    dct:isReferencedBy F2021L00310: ;
    rdfs:comment "9 18  Decisions that may be made by operation of computer program - Abrievated Graph Key: I219"@en-AU ;
    skos:definition "9 18  Decisions that may be made by operation of computer program"@en-AU ;
    skos:narrower F2021L00310:218 ;
    skos:prefLabel "Item I219"@en-AU ;
    dcat:accessURL <https://www.legislation.gov.au/F2021L00310/2023-08-04/2023-08-04/text/1/epub/OEBPS/document_1/document_1.html#_Toc145601545> ;
    dcat:landingPage "https://www.legislation.gov.au/F2021L00310/2023-08-04/2023-08-04/text/1/epub/OEBPS/document_1/document_1.html#_Toc145601545"^^xsd:anyURI ;
    dcat:theme legcons:Item .

F2021L00310:22 a legcons:Item,
        owl:Class,
        dcat:Resource ;
    rdfs:label "Item - I22 2 5  Application of this Part"@en-AU ;
    dct:isPartOf F2021L00310:21 ;
    dct:isReferencedBy F2021L00310: ;
    rdfs:comment "2 5  Application of this Part - Abrievated Graph Key: I22"@en-AU ;
    skos:definition "2 5  Application of this Part"@en-AU ;
    skos:narrower F2021L00310:21 ;
    skos:prefLabel "Item I22"@en-AU ;
    dcat:accessURL <https://www.legislation.gov.au/F2021L00310/2023-08-04/2023-08-04/text/1/epub/OEBPS/document_1/document_1.html#_Toc145601348> ;
    dcat:landingPage "https://www.legislation.gov.au/F2021L00310/2023-08-04/2023-08-04/text/1/epub/OEBPS/document_1/document_1.html#_Toc145601348"^^xsd:anyURI ;
    dcat:theme legcons:Item .

F2021L00310:222 a legcons:Item,
        owl:Class,
        dcat:Resource ;
    rdfs:label "Item - I222 9 19  Requirement to be third party authorised officerfit and proper person etc"@en-AU ;
    dct:isPartOf F2021L00310:221 ;
    dct:isReferencedBy F2021L00310: ;
    rdfs:comment "9 19  Requirement to be third party authorised officerfit and proper person etc - Abrievated Graph Key: I222"@en-AU ;
    skos:definition "9 19  Requirement to be third party authorised officerfit and proper person etc"@en-AU ;
    skos:narrower F2021L00310:221 ;
    skos:prefLabel "Item I222"@en-AU ;
    dcat:accessURL <https://www.legislation.gov.au/F2021L00310/2023-08-04/2023-08-04/text/1/epub/OEBPS/document_1/document_1.html#_Toc145601548> ;
    dcat:landingPage "https://www.legislation.gov.au/F2021L00310/2023-08-04/2023-08-04/text/1/epub/OEBPS/document_1/document_1.html#_Toc145601548"^^xsd:anyURI ;
    dcat:theme legcons:Item .

F2021L00310:224 a legcons:Item,
        owl:Class,
        dcat:Resource ;
    rdfs:label "Item - I224 9 20  Purpose of this Division"@en-AU ;
    dct:isPartOf F2021L00310:223 ;
    dct:isReferencedBy F2021L00310: ;
    rdfs:comment "9 20  Purpose of this Division - Abrievated Graph Key: I224"@en-AU ;
    skos:definition "9 20  Purpose of this Division"@en-AU ;
    skos:narrower F2021L00310:223 ;
    skos:prefLabel "Item I224"@en-AU ;
    dcat:accessURL <https://www.legislation.gov.au/F2021L00310/2023-08-04/2023-08-04/text/1/epub/OEBPS/document_1/document_1.html#_Toc145601550> ;
    dcat:landingPage "https://www.legislation.gov.au/F2021L00310/2023-08-04/2023-08-04/text/1/epub/OEBPS/document_1/document_1.html#_Toc145601550"^^xsd:anyURI ;
    dcat:theme legcons:Item .

F2021L00310:225 a legcons:Item,
        owl:Class,
        dcat:Resource ;
    rdfs:label "Item - I225 9 21  Applying admission decisions"@en-AU ;
    dct:isPartOf F2021L00310:223 ;
    dct:isReferencedBy F2021L00310: ;
    rdfs:comment "9 21  Applying admission decisions - Abrievated Graph Key: I225"@en-AU ;
    skos:definition "9 21  Applying admission decisions"@en-AU ;
    skos:narrower F2021L00310:223 ;
    skos:prefLabel "Item I225"@en-AU ;
    dcat:accessURL <https://www.legislation.gov.au/F2021L00310/2023-08-04/2023-08-04/text/1/epub/OEBPS/document_1/document_1.html#_Toc145601551> ;
    dcat:landingPage "https://www.legislation.gov.au/F2021L00310/2023-08-04/2023-08-04/text/1/epub/OEBPS/document_1/document_1.html#_Toc145601551"^^xsd:anyURI ;
    dcat:theme legcons:Item .

F2021L00310:226 a legcons:Item,
        owl:Class,
        dcat:Resource ;
    rdfs:label "Item - I226 9 22  Inspections of poultry for slaughter and applying ante mortem dispositions"@en-AU ;
    dct:isPartOf F2021L00310:223 ;
    dct:isReferencedBy F2021L00310: ;
    rdfs:comment "9 22  Inspections of poultry for slaughter and applying ante mortem dispositions - Abrievated Graph Key: I226"@en-AU ;
    skos:definition "9 22  Inspections of poultry for slaughter and applying ante mortem dispositions"@en-AU ;
    skos:narrower F2021L00310:223 ;
    skos:prefLabel "Item I226"@en-AU ;
    dcat:accessURL <https://www.legislation.gov.au/F2021L00310/2023-08-04/2023-08-04/text/1/epub/OEBPS/document_1/document_1.html#_Toc145601552> ;
    dcat:landingPage "https://www.legislation.gov.au/F2021L00310/2023-08-04/2023-08-04/text/1/epub/OEBPS/document_1/document_1.html#_Toc145601552"^^xsd:anyURI ;
    dcat:theme legcons:Item .

F2021L00310:227 a legcons:Item,
        owl:Class,
        dcat:Resource ;
    rdfs:label "Item - I227 9 23  Inspections of carcases and carcase parts and applying post mortem dispositions"@en-AU ;
    dct:isPartOf F2021L00310:223 ;
    dct:isReferencedBy F2021L00310: ;
    rdfs:comment "9 23  Inspections of carcases and carcase parts and applying post mortem dispositions - Abrievated Graph Key: I227"@en-AU ;
    skos:definition "9 23  Inspections of carcases and carcase parts and applying post mortem dispositions"@en-AU ;
    skos:narrower F2021L00310:223 ;
    skos:prefLabel "Item I227"@en-AU ;
    dcat:accessURL <https://www.legislation.gov.au/F2021L00310/2023-08-04/2023-08-04/text/1/epub/OEBPS/document_1/document_1.html#_Toc145601553> ;
    dcat:landingPage "https://www.legislation.gov.au/F2021L00310/2023-08-04/2023-08-04/text/1/epub/OEBPS/document_1/document_1.html#_Toc145601553"^^xsd:anyURI ;
    dcat:theme legcons:Item .

F2021L00310:228 a legcons:Item,
        owl:Class,
        dcat:Resource ;
    rdfs:label "Item - I228 9 24  Inspections of poultry meat and poultry meat products and applying dispositions"@en-AU ;
    dct:isPartOf F2021L00310:223 ;
    dct:isReferencedBy F2021L00310: ;
    rdfs:comment "9 24  Inspections of poultry meat and poultry meat products and applying dispositions - Abrievated Graph Key: I228"@en-AU ;
    skos:definition "9 24  Inspections of poultry meat and poultry meat products and applying dispositions"@en-AU ;
    skos:narrower F2021L00310:223 ;
    skos:prefLabel "Item I228"@en-AU ;
    dcat:accessURL <https://www.legislation.gov.au/F2021L00310/2023-08-04/2023-08-04/text/1/epub/OEBPS/document_1/document_1.html#_Toc145601554> ;
    dcat:landingPage "https://www.legislation.gov.au/F2021L00310/2023-08-04/2023-08-04/text/1/epub/OEBPS/document_1/document_1.html#_Toc145601554"^^xsd:anyURI ;
    dcat:theme legcons:Item .

F2021L00310:229 a legcons:Item,
        owl:Class,
        dcat:Resource ;
    rdfs:label "Item - I229 9 25  Applying decisions or dispositions subject to conditions and variation"@en-AU ;
    dct:isPartOf F2021L00310:223 ;
    dct:isReferencedBy F2021L00310: ;
    rdfs:comment "9 25  Applying decisions or dispositions subject to conditions and variation - Abrievated Graph Key: I229"@en-AU ;
    skos:definition "9 25  Applying decisions or dispositions subject to conditions and variation"@en-AU ;
    skos:narrower F2021L00310:223 ;
    skos:prefLabel "Item I229"@en-AU ;
    dcat:accessURL <https://www.legislation.gov.au/F2021L00310/2023-08-04/2023-08-04/text/1/epub/OEBPS/document_1/document_1.html#_Toc145601555> ;
    dcat:landingPage "https://www.legislation.gov.au/F2021L00310/2023-08-04/2023-08-04/text/1/epub/OEBPS/document_1/document_1.html#_Toc145601555"^^xsd:anyURI ;
    dcat:theme legcons:Item .

F2021L00310:23 a legcons:Item,
        owl:Class,
        dcat:Resource ;
    rdfs:label "Item - I23 2 6  Period for making application for exemption"@en-AU ;
    dct:isPartOf F2021L00310:21 ;
    dct:isReferencedBy F2021L00310: ;
    rdfs:comment "2 6  Period for making application for exemption - Abrievated Graph Key: I23"@en-AU ;
    skos:definition "2 6  Period for making application for exemption"@en-AU ;
    skos:narrower F2021L00310:21 ;
    skos:prefLabel "Item I23"@en-AU ;
    dcat:accessURL <https://www.legislation.gov.au/F2021L00310/2023-08-04/2023-08-04/text/1/epub/OEBPS/document_1/document_1.html#_Toc145601349> ;
    dcat:landingPage "https://www.legislation.gov.au/F2021L00310/2023-08-04/2023-08-04/text/1/epub/OEBPS/document_1/document_1.html#_Toc145601349"^^xsd:anyURI ;
    dcat:theme legcons:Item .

F2021L00310:230 a legcons:Item,
        owl:Class,
        dcat:Resource ;
    rdfs:label "Item - I230 9 26  Stopping chain of operations temporarily or controlling rate of operations"@en-AU ;
    dct:isPartOf F2021L00310:223 ;
    dct:isReferencedBy F2021L00310: ;
    rdfs:comment "9 26  Stopping chain of operations temporarily or controlling rate of operations - Abrievated Graph Key: I230"@en-AU ;
    skos:definition "9 26  Stopping chain of operations temporarily or controlling rate of operations"@en-AU ;
    skos:narrower F2021L00310:223 ;
    skos:prefLabel "Item I230"@en-AU ;
    dcat:accessURL <https://www.legislation.gov.au/F2021L00310/2023-08-04/2023-08-04/text/1/epub/OEBPS/document_1/document_1.html#_Toc145601556> ;
    dcat:landingPage "https://www.legislation.gov.au/F2021L00310/2023-08-04/2023-08-04/text/1/epub/OEBPS/document_1/document_1.html#_Toc145601556"^^xsd:anyURI ;
    dcat:theme legcons:Item .

F2021L00310:231 a legcons:Item,
        owl:Class,
        dcat:Resource ;
    rdfs:label "Item - I231 9 27  Inspecting establishments and securing areas facilities equipment or other things"@en-AU ;
    dct:isPartOf F2021L00310:223 ;
    dct:isReferencedBy F2021L00310: ;
    rdfs:comment "9 27  Inspecting establishments and securing areas facilities equipment or other things - Abrievated Graph Key: I231"@en-AU ;
    skos:definition "9 27  Inspecting establishments and securing areas facilities equipment or other things"@en-AU ;
    skos:narrower F2021L00310:223 ;
    skos:prefLabel "Item I231"@en-AU ;
    dcat:accessURL <https://www.legislation.gov.au/F2021L00310/2023-08-04/2023-08-04/text/1/epub/OEBPS/document_1/document_1.html#_Toc145601557> ;
    dcat:landingPage "https://www.legislation.gov.au/F2021L00310/2023-08-04/2023-08-04/text/1/epub/OEBPS/document_1/document_1.html#_Toc145601557"^^xsd:anyURI ;
    dcat:theme legcons:Item .

F2021L00310:232 a legcons:Item,
        owl:Class,
        dcat:Resource ;
    rdfs:label "Item - I232 9 28  Securing and identifying establishment or conveyance etc"@en-AU ;
    dct:isPartOf F2021L00310:223 ;
    dct:isReferencedBy F2021L00310: ;
    rdfs:comment "9 28  Securing and identifying establishment or conveyance etc - Abrievated Graph Key: I232"@en-AU ;
    skos:definition "9 28  Securing and identifying establishment or conveyance etc"@en-AU ;
    skos:narrower F2021L00310:223 ;
    skos:prefLabel "Item I232"@en-AU ;
    dcat:accessURL <https://www.legislation.gov.au/F2021L00310/2023-08-04/2023-08-04/text/1/epub/OEBPS/document_1/document_1.html#_Toc145601558> ;
    dcat:landingPage "https://www.legislation.gov.au/F2021L00310/2023-08-04/2023-08-04/text/1/epub/OEBPS/document_1/document_1.html#_Toc145601558"^^xsd:anyURI ;
    dcat:theme legcons:Item .

F2021L00310:233 a legcons:Item,
        owl:Class,
        dcat:Resource ;
    rdfs:label "Item - I233 9 29  Interference with identified establishment or conveyance etc"@en-AU ;
    dct:isPartOf F2021L00310:223 ;
    dct:isReferencedBy F2021L00310: ;
    rdfs:comment "9 29  Interference with identified establishment or conveyance etc - Abrievated Graph Key: I233"@en-AU ;
    skos:definition "9 29  Interference with identified establishment or conveyance etc"@en-AU ;
    skos:narrower F2021L00310:223 ;
    skos:prefLabel "Item I233"@en-AU ;
    dcat:accessURL <https://www.legislation.gov.au/F2021L00310/2023-08-04/2023-08-04/text/1/epub/OEBPS/document_1/document_1.html#_Toc145601559> ;
    dcat:landingPage "https://www.legislation.gov.au/F2021L00310/2023-08-04/2023-08-04/text/1/epub/OEBPS/document_1/document_1.html#_Toc145601559"^^xsd:anyURI ;
    dcat:theme legcons:Item .

F2021L00310:234 a legcons:Item,
        owl:Class,
        dcat:Resource ;
    rdfs:label "Item - I234 9 30  Powers where integrity of prescribed poultry meat or poultry meat products may not be able to be ensured"@en-AU ;
    dct:isPartOf F2021L00310:223 ;
    dct:isReferencedBy F2021L00310: ;
    rdfs:comment "9 30  Powers where integrity of prescribed poultry meat or poultry meat products may not be able to be ensured - Abrievated Graph Key: I234"@en-AU ;
    skos:definition "9 30  Powers where integrity of prescribed poultry meat or poultry meat products may not be able to be ensured"@en-AU ;
    skos:narrower F2021L00310:223 ;
    skos:prefLabel "Item I234"@en-AU ;
    dcat:accessURL <https://www.legislation.gov.au/F2021L00310/2023-08-04/2023-08-04/text/1/epub/OEBPS/document_1/document_1.html#_Toc145601560> ;
    dcat:landingPage "https://www.legislation.gov.au/F2021L00310/2023-08-04/2023-08-04/text/1/epub/OEBPS/document_1/document_1.html#_Toc145601560"^^xsd:anyURI ;
    dcat:theme legcons:Item .

F2021L00310:235 a legcons:Item,
        owl:Class,
        dcat:Resource ;
    rdfs:label "Item - I235 9 31  Giving certificate of condemnation"@en-AU ;
    dct:isPartOf F2021L00310:223 ;
    dct:isReferencedBy F2021L00310: ;
    rdfs:comment "9 31  Giving certificate of condemnation - Abrievated Graph Key: I235"@en-AU ;
    skos:definition "9 31  Giving certificate of condemnation"@en-AU ;
    skos:narrower F2021L00310:223 ;
    skos:prefLabel "Item I235"@en-AU ;
    dcat:accessURL <https://www.legislation.gov.au/F2021L00310/2023-08-04/2023-08-04/text/1/epub/OEBPS/document_1/document_1.html#_Toc145601561> ;
    dcat:landingPage "https://www.legislation.gov.au/F2021L00310/2023-08-04/2023-08-04/text/1/epub/OEBPS/document_1/document_1.html#_Toc145601561"^^xsd:anyURI ;
    dcat:theme legcons:Item .

F2021L00310:237 a legcons:Item,
        owl:Class,
        dcat:Resource ;
    rdfs:label "Item - I237 9 32  Other grounds for giving direction"@en-AU ;
    dct:isPartOf F2021L00310:236 ;
    dct:isReferencedBy F2021L00310: ;
    rdfs:comment "9 32  Other grounds for giving direction - Abrievated Graph Key: I237"@en-AU ;
    skos:definition "9 32  Other grounds for giving direction"@en-AU ;
    skos:narrower F2021L00310:236 ;
    skos:prefLabel "Item I237"@en-AU ;
    dcat:accessURL <https://www.legislation.gov.au/F2021L00310/2023-08-04/2023-08-04/text/1/epub/OEBPS/document_1/document_1.html#_Toc145601563> ;
    dcat:landingPage "https://www.legislation.gov.au/F2021L00310/2023-08-04/2023-08-04/text/1/epub/OEBPS/document_1/document_1.html#_Toc145601563"^^xsd:anyURI ;
    dcat:theme legcons:Item .

F2021L00310:239 a legcons:Item,
        owl:Class,
        dcat:Resource ;
    rdfs:label "Item - I239 9 33  Circumstances in which identity card need not be carried"@en-AU ;
    dct:isPartOf F2021L00310:238 ;
    dct:isReferencedBy F2021L00310: ;
    rdfs:comment "9 33  Circumstances in which identity card need not be carried - Abrievated Graph Key: I239"@en-AU ;
    skos:definition "9 33  Circumstances in which identity card need not be carried"@en-AU ;
    skos:narrower F2021L00310:238 ;
    skos:prefLabel "Item I239"@en-AU ;
    dcat:accessURL <https://www.legislation.gov.au/F2021L00310/2023-08-04/2023-08-04/text/1/epub/OEBPS/document_1/document_1.html#_Toc145601565> ;
    dcat:landingPage "https://www.legislation.gov.au/F2021L00310/2023-08-04/2023-08-04/text/1/epub/OEBPS/document_1/document_1.html#_Toc145601565"^^xsd:anyURI ;
    dcat:theme legcons:Item .

F2021L00310:24 a legcons:Item,
        owl:Class,
        dcat:Resource ;
    rdfs:label "Item - I24 2 7  Conditions of exemptionmatters to which Secretary must have regard"@en-AU ;
    dct:isPartOf F2021L00310:21 ;
    dct:isReferencedBy F2021L00310: ;
    rdfs:comment "2 7  Conditions of exemptionmatters to which Secretary must have regard - Abrievated Graph Key: I24"@en-AU ;
    skos:definition "2 7  Conditions of exemptionmatters to which Secretary must have regard"@en-AU ;
    skos:narrower F2021L00310:21 ;
    skos:prefLabel "Item I24"@en-AU ;
    dcat:accessURL <https://www.legislation.gov.au/F2021L00310/2023-08-04/2023-08-04/text/1/epub/OEBPS/document_1/document_1.html#_Toc145601350> ;
    dcat:landingPage "https://www.legislation.gov.au/F2021L00310/2023-08-04/2023-08-04/text/1/epub/OEBPS/document_1/document_1.html#_Toc145601350"^^xsd:anyURI ;
    dcat:theme legcons:Item .

F2021L00310:241 a legcons:Item,
        owl:Class,
        dcat:Resource ;
    rdfs:label "Item - I241 10 1  Samples taken in exercising monitoring or investigation powers"@en-AU ;
    dct:isPartOf F2021L00310:240 ;
    dct:isReferencedBy F2021L00310: ;
    rdfs:comment "10 1  Samples taken in exercising monitoring or investigation powers - Abrievated Graph Key: I241"@en-AU ;
    skos:definition "10 1  Samples taken in exercising monitoring or investigation powers"@en-AU ;
    skos:narrower F2021L00310:240 ;
    skos:prefLabel "Item I241"@en-AU ;
    dcat:accessURL <https://www.legislation.gov.au/F2021L00310/2023-08-04/2023-08-04/text/1/epub/OEBPS/document_1/document_1.html#_Toc145601567> ;
    dcat:landingPage "https://www.legislation.gov.au/F2021L00310/2023-08-04/2023-08-04/text/1/epub/OEBPS/document_1/document_1.html#_Toc145601567"^^xsd:anyURI ;
    dcat:theme legcons:Item .

F2021L00310:242 a legcons:Item,
        owl:Class,
        dcat:Resource ;
    rdfs:label "Item - I242 10 2  Dealing with things seized in exercising investigation powers"@en-AU ;
    dct:isPartOf F2021L00310:240 ;
    dct:isReferencedBy F2021L00310: ;
    rdfs:comment "10 2  Dealing with things seized in exercising investigation powers - Abrievated Graph Key: I242"@en-AU ;
    skos:definition "10 2  Dealing with things seized in exercising investigation powers"@en-AU ;
    skos:narrower F2021L00310:240 ;
    skos:prefLabel "Item I242"@en-AU ;
    dcat:accessURL <https://www.legislation.gov.au/F2021L00310/2023-08-04/2023-08-04/text/1/epub/OEBPS/document_1/document_1.html#_Toc145601568> ;
    dcat:landingPage "https://www.legislation.gov.au/F2021L00310/2023-08-04/2023-08-04/text/1/epub/OEBPS/document_1/document_1.html#_Toc145601568"^^xsd:anyURI ;
    dcat:theme legcons:Item .

F2021L00310:245 a legcons:Item,
        owl:Class,
        dcat:Resource ;
    rdfs:label "Item - I245 11 1  Reviewable decisions"@en-AU ;
    dct:isPartOf F2021L00310:244 ;
    dct:isReferencedBy F2021L00310: ;
    rdfs:comment "11 1  Reviewable decisions - Abrievated Graph Key: I245"@en-AU ;
    skos:definition "11 1  Reviewable decisions"@en-AU ;
    skos:narrower F2021L00310:244 ;
    skos:prefLabel "Item I245"@en-AU ;
    dcat:accessURL <https://www.legislation.gov.au/F2021L00310/2023-08-04/2023-08-04/text/1/epub/OEBPS/document_1/document_1.html#_Toc145601571> ;
    dcat:landingPage "https://www.legislation.gov.au/F2021L00310/2023-08-04/2023-08-04/text/1/epub/OEBPS/document_1/document_1.html#_Toc145601571"^^xsd:anyURI ;
    dcat:theme legcons:Item .

F2021L00310:247 a legcons:Item,
        owl:Class,
        dcat:Resource ;
    rdfs:label "Item - I247 11 2  Purpose of this Part"@en-AU ;
    dct:isPartOf F2021L00310:246 ;
    dct:isReferencedBy F2021L00310: ;
    rdfs:comment "11 2  Purpose of this Part - Abrievated Graph Key: I247"@en-AU ;
    skos:definition "11 2  Purpose of this Part"@en-AU ;
    skos:narrower F2021L00310:246 ;
    skos:prefLabel "Item I247"@en-AU ;
    dcat:accessURL <https://www.legislation.gov.au/F2021L00310/2023-08-04/2023-08-04/text/1/epub/OEBPS/document_1/document_1.html#_Toc145601573> ;
    dcat:landingPage "https://www.legislation.gov.au/F2021L00310/2023-08-04/2023-08-04/text/1/epub/OEBPS/document_1/document_1.html#_Toc145601573"^^xsd:anyURI ;
    dcat:theme legcons:Item .

F2021L00310:248 a legcons:Item,
        owl:Class,
        dcat:Resource ;
    rdfs:label "Item - I248 11 3  General requirements for records"@en-AU ;
    dct:isPartOf F2021L00310:246 ;
    dct:isReferencedBy F2021L00310: ;
    rdfs:comment "11 3  General requirements for records - Abrievated Graph Key: I248"@en-AU ;
    skos:definition "11 3  General requirements for records"@en-AU ;
    skos:narrower F2021L00310:246 ;
    skos:prefLabel "Item I248"@en-AU ;
    dcat:accessURL <https://www.legislation.gov.au/F2021L00310/2023-08-04/2023-08-04/text/1/epub/OEBPS/document_1/document_1.html#_Toc145601574> ;
    dcat:landingPage "https://www.legislation.gov.au/F2021L00310/2023-08-04/2023-08-04/text/1/epub/OEBPS/document_1/document_1.html#_Toc145601574"^^xsd:anyURI ;
    dcat:theme legcons:Item .

F2021L00310:249 a legcons:Item,
        owl:Class,
        dcat:Resource ;
    rdfs:label "Item - I249 11 4  Government certificates"@en-AU ;
    dct:isPartOf F2021L00310:246 ;
    dct:isReferencedBy F2021L00310: ;
    rdfs:comment "11 4  Government certificates - Abrievated Graph Key: I249"@en-AU ;
    skos:definition "11 4  Government certificates"@en-AU ;
    skos:narrower F2021L00310:246 ;
    skos:prefLabel "Item I249"@en-AU ;
    dcat:accessURL <https://www.legislation.gov.au/F2021L00310/2023-08-04/2023-08-04/text/1/epub/OEBPS/document_1/document_1.html#_Toc145601575> ;
    dcat:landingPage "https://www.legislation.gov.au/F2021L00310/2023-08-04/2023-08-04/text/1/epub/OEBPS/document_1/document_1.html#_Toc145601575"^^xsd:anyURI ;
    dcat:theme legcons:Item .

F2021L00310:25 a legcons:Item,
        owl:Class,
        dcat:Resource ;
    rdfs:label "Item - I25 2 8  Period of effect of exemption"@en-AU ;
    dct:isPartOf F2021L00310:21 ;
    dct:isReferencedBy F2021L00310: ;
    rdfs:comment "2 8  Period of effect of exemption - Abrievated Graph Key: I25"@en-AU ;
    skos:definition "2 8  Period of effect of exemption"@en-AU ;
    skos:narrower F2021L00310:21 ;
    skos:prefLabel "Item I25"@en-AU ;
    dcat:accessURL <https://www.legislation.gov.au/F2021L00310/2023-08-04/2023-08-04/text/1/epub/OEBPS/document_1/document_1.html#_Toc145601351> ;
    dcat:landingPage "https://www.legislation.gov.au/F2021L00310/2023-08-04/2023-08-04/text/1/epub/OEBPS/document_1/document_1.html#_Toc145601351"^^xsd:anyURI ;
    dcat:theme legcons:Item .

F2021L00310:250 a legcons:Item,
        owl:Class,
        dcat:Resource ;
    rdfs:label "Item - I250 11 5  Export permits"@en-AU ;
    dct:isPartOf F2021L00310:246 ;
    dct:isReferencedBy F2021L00310: ;
    rdfs:comment "11 5  Export permits - Abrievated Graph Key: I250"@en-AU ;
    skos:definition "11 5  Export permits"@en-AU ;
    skos:narrower F2021L00310:246 ;
    skos:prefLabel "Item I250"@en-AU ;
    dcat:accessURL <https://www.legislation.gov.au/F2021L00310/2023-08-04/2023-08-04/text/1/epub/OEBPS/document_1/document_1.html#_Toc145601576> ;
    dcat:landingPage "https://www.legislation.gov.au/F2021L00310/2023-08-04/2023-08-04/text/1/epub/OEBPS/document_1/document_1.html#_Toc145601576"^^xsd:anyURI ;
    dcat:theme legcons:Item .

F2021L00310:251 a legcons:Item,
        owl:Class,
        dcat:Resource ;
    rdfs:label "Item - I251 11 6  Records to be retained by exporter"@en-AU ;
    dct:isPartOf F2021L00310:246 ;
    dct:isReferencedBy F2021L00310: ;
    rdfs:comment "11 6  Records to be retained by exporter - Abrievated Graph Key: I251"@en-AU ;
    skos:definition "11 6  Records to be retained by exporter"@en-AU ;
    skos:narrower F2021L00310:246 ;
    skos:prefLabel "Item I251"@en-AU ;
    dcat:accessURL <https://www.legislation.gov.au/F2021L00310/2023-08-04/2023-08-04/text/1/epub/OEBPS/document_1/document_1.html#_Toc145601577> ;
    dcat:landingPage "https://www.legislation.gov.au/F2021L00310/2023-08-04/2023-08-04/text/1/epub/OEBPS/document_1/document_1.html#_Toc145601577"^^xsd:anyURI ;
    dcat:theme legcons:Item .

F2021L00310:252 a legcons:Item,
        owl:Class,
        dcat:Resource ;
    rdfs:label "Item - I252 11 7  Records to be retained by occupier of registered establishment"@en-AU ;
    dct:isPartOf F2021L00310:246 ;
    dct:isReferencedBy F2021L00310: ;
    rdfs:comment "11 7  Records to be retained by occupier of registered establishment - Abrievated Graph Key: I252"@en-AU ;
    skos:definition "11 7  Records to be retained by occupier of registered establishment"@en-AU ;
    skos:narrower F2021L00310:246 ;
    skos:prefLabel "Item I252"@en-AU ;
    dcat:accessURL <https://www.legislation.gov.au/F2021L00310/2023-08-04/2023-08-04/text/1/epub/OEBPS/document_1/document_1.html#_Toc145601578> ;
    dcat:landingPage "https://www.legislation.gov.au/F2021L00310/2023-08-04/2023-08-04/text/1/epub/OEBPS/document_1/document_1.html#_Toc145601578"^^xsd:anyURI ;
    dcat:theme legcons:Item .

F2021L00310:253 a legcons:Item,
        owl:Class,
        dcat:Resource ;
    rdfs:label "Item - I253 11 8  Records to be retained by holder of approved arrangement"@en-AU ;
    dct:isPartOf F2021L00310:246 ;
    dct:isReferencedBy F2021L00310: ;
    rdfs:comment "11 8  Records to be retained by holder of approved arrangement - Abrievated Graph Key: I253"@en-AU ;
    skos:definition "11 8  Records to be retained by holder of approved arrangement"@en-AU ;
    skos:narrower F2021L00310:246 ;
    skos:prefLabel "Item I253"@en-AU ;
    dcat:accessURL <https://www.legislation.gov.au/F2021L00310/2023-08-04/2023-08-04/text/1/epub/OEBPS/document_1/document_1.html#_Toc145601579> ;
    dcat:landingPage "https://www.legislation.gov.au/F2021L00310/2023-08-04/2023-08-04/text/1/epub/OEBPS/document_1/document_1.html#_Toc145601579"^^xsd:anyURI ;
    dcat:theme legcons:Item .

F2021L00310:254 a legcons:Item,
        owl:Class,
        dcat:Resource ;
    rdfs:label "Item - I254 11 9  Records relating to official marks"@en-AU ;
    dct:isPartOf F2021L00310:246 ;
    dct:isReferencedBy F2021L00310: ;
    rdfs:comment "11 9  Records relating to official marks - Abrievated Graph Key: I254"@en-AU ;
    skos:definition "11 9  Records relating to official marks"@en-AU ;
    skos:narrower F2021L00310:246 ;
    skos:prefLabel "Item I254"@en-AU ;
    dcat:accessURL <https://www.legislation.gov.au/F2021L00310/2023-08-04/2023-08-04/text/1/epub/OEBPS/document_1/document_1.html#_Toc145601580> ;
    dcat:landingPage "https://www.legislation.gov.au/F2021L00310/2023-08-04/2023-08-04/text/1/epub/OEBPS/document_1/document_1.html#_Toc145601580"^^xsd:anyURI ;
    dcat:theme legcons:Item .

F2021L00310:255 a legcons:Item,
        owl:Class,
        dcat:Resource ;
    rdfs:label "Item - I255 11 10  Records relating to official marking devices"@en-AU ;
    dct:isPartOf F2021L00310:246 ;
    dct:isReferencedBy F2021L00310: ;
    rdfs:comment "11 10  Records relating to official marking devices - Abrievated Graph Key: I255"@en-AU ;
    skos:definition "11 10  Records relating to official marking devices"@en-AU ;
    skos:narrower F2021L00310:246 ;
    skos:prefLabel "Item I255"@en-AU ;
    dcat:accessURL <https://www.legislation.gov.au/F2021L00310/2023-08-04/2023-08-04/text/1/epub/OEBPS/document_1/document_1.html#_Toc145601581> ;
    dcat:landingPage "https://www.legislation.gov.au/F2021L00310/2023-08-04/2023-08-04/text/1/epub/OEBPS/document_1/document_1.html#_Toc145601581"^^xsd:anyURI ;
    dcat:theme legcons:Item .

F2021L00310:256 a legcons:Item,
        owl:Class,
        dcat:Resource ;
    rdfs:label "Item - I256 11 11  Records must not be altered or defaced during retention period"@en-AU ;
    dct:isPartOf F2021L00310:246 ;
    dct:isReferencedBy F2021L00310: ;
    rdfs:comment "11 11  Records must not be altered or defaced during retention period - Abrievated Graph Key: I256"@en-AU ;
    skos:definition "11 11  Records must not be altered or defaced during retention period"@en-AU ;
    skos:narrower F2021L00310:246 ;
    skos:prefLabel "Item I256"@en-AU ;
    dcat:accessURL <https://www.legislation.gov.au/F2021L00310/2023-08-04/2023-08-04/text/1/epub/OEBPS/document_1/document_1.html#_Toc145601582> ;
    dcat:landingPage "https://www.legislation.gov.au/F2021L00310/2023-08-04/2023-08-04/text/1/epub/OEBPS/document_1/document_1.html#_Toc145601582"^^xsd:anyURI ;
    dcat:theme legcons:Item .

F2021L00310:258 a legcons:Item,
        owl:Class,
        dcat:Resource ;
    rdfs:label "Item - I258 11 12  Storage of samples"@en-AU ;
    dct:isPartOf F2021L00310:257 ;
    dct:isReferencedBy F2021L00310: ;
    rdfs:comment "11 12  Storage of samples - Abrievated Graph Key: I258"@en-AU ;
    skos:definition "11 12  Storage of samples"@en-AU ;
    skos:narrower F2021L00310:257 ;
    skos:prefLabel "Item I258"@en-AU ;
    dcat:accessURL <https://www.legislation.gov.au/F2021L00310/2023-08-04/2023-08-04/text/1/epub/OEBPS/document_1/document_1.html#_Toc145601584> ;
    dcat:landingPage "https://www.legislation.gov.au/F2021L00310/2023-08-04/2023-08-04/text/1/epub/OEBPS/document_1/document_1.html#_Toc145601584"^^xsd:anyURI ;
    dcat:theme legcons:Item .

F2021L00310:26 a legcons:Item,
        owl:Class,
        dcat:Resource ;
    rdfs:label "Item - I26 2 9  Variation of conditions of exemptionmatters to which Secretary must have regard"@en-AU ;
    dct:isPartOf F2021L00310:21 ;
    dct:isReferencedBy F2021L00310: ;
    rdfs:comment "2 9  Variation of conditions of exemptionmatters to which Secretary must have regard - Abrievated Graph Key: I26"@en-AU ;
    skos:definition "2 9  Variation of conditions of exemptionmatters to which Secretary must have regard"@en-AU ;
    skos:narrower F2021L00310:21 ;
    skos:prefLabel "Item I26"@en-AU ;
    dcat:accessURL <https://www.legislation.gov.au/F2021L00310/2023-08-04/2023-08-04/text/1/epub/OEBPS/document_1/document_1.html#_Toc145601352> ;
    dcat:landingPage "https://www.legislation.gov.au/F2021L00310/2023-08-04/2023-08-04/text/1/epub/OEBPS/document_1/document_1.html#_Toc145601352"^^xsd:anyURI ;
    dcat:theme legcons:Item .

F2021L00310:260 a legcons:Item,
        owl:Class,
        dcat:Resource ;
    rdfs:label "Item - I260 11 13  Division of compensation between owners"@en-AU ;
    dct:isPartOf F2021L00310:259 ;
    dct:isReferencedBy F2021L00310: ;
    rdfs:comment "11 13  Division of compensation between owners - Abrievated Graph Key: I260"@en-AU ;
    skos:definition "11 13  Division of compensation between owners"@en-AU ;
    skos:narrower F2021L00310:259 ;
    skos:prefLabel "Item I260"@en-AU ;
    dcat:accessURL <https://www.legislation.gov.au/F2021L00310/2023-08-04/2023-08-04/text/1/epub/OEBPS/document_1/document_1.html#_Toc145601586> ;
    dcat:landingPage "https://www.legislation.gov.au/F2021L00310/2023-08-04/2023-08-04/text/1/epub/OEBPS/document_1/document_1.html#_Toc145601586"^^xsd:anyURI ;
    dcat:theme legcons:Item .

F2021L00310:261 a legcons:Item,
        owl:Class,
        dcat:Resource ;
    rdfs:label "Item - I261 11 14  Amount of compensation"@en-AU ;
    dct:isPartOf F2021L00310:259 ;
    dct:isReferencedBy F2021L00310: ;
    rdfs:comment "11 14  Amount of compensation - Abrievated Graph Key: I261"@en-AU ;
    skos:definition "11 14  Amount of compensation"@en-AU ;
    skos:narrower F2021L00310:259 ;
    skos:prefLabel "Item I261"@en-AU ;
    dcat:accessURL <https://www.legislation.gov.au/F2021L00310/2023-08-04/2023-08-04/text/1/epub/OEBPS/document_1/document_1.html#_Toc145601587> ;
    dcat:landingPage "https://www.legislation.gov.au/F2021L00310/2023-08-04/2023-08-04/text/1/epub/OEBPS/document_1/document_1.html#_Toc145601587"^^xsd:anyURI ;
    dcat:theme legcons:Item .

F2021L00310:263 a legcons:Item,
        owl:Class,
        dcat:Resource ;
    rdfs:label "Item - I263 11 15  Circumstances in which relevant Commonwealth liability of a person is taken to have been paid"@en-AU ;
    dct:isPartOf F2021L00310:262 ;
    dct:isReferencedBy F2021L00310: ;
    rdfs:comment "11 15  Circumstances in which relevant Commonwealth liability of a person is taken to have been paid - Abrievated Graph Key: I263"@en-AU ;
    skos:definition "11 15  Circumstances in which relevant Commonwealth liability of a person is taken to have been paid"@en-AU ;
    skos:narrower F2021L00310:262 ;
    skos:prefLabel "Item I263"@en-AU ;
    dcat:accessURL <https://www.legislation.gov.au/F2021L00310/2023-08-04/2023-08-04/text/1/epub/OEBPS/document_1/document_1.html#_Toc145601589> ;
    dcat:landingPage "https://www.legislation.gov.au/F2021L00310/2023-08-04/2023-08-04/text/1/epub/OEBPS/document_1/document_1.html#_Toc145601589"^^xsd:anyURI ;
    dcat:theme legcons:Item .

F2021L00310:266 a legcons:Item,
        owl:Class,
        dcat:Resource ;
    rdfs:label "Item - I266 12 1  Definitions"@en-AU ;
    dct:isPartOf F2021L00310:265 ;
    dct:isReferencedBy F2021L00310: ;
    rdfs:comment "12 1  Definitions - Abrievated Graph Key: I266"@en-AU ;
    skos:definition "12 1  Definitions"@en-AU ;
    skos:narrower F2021L00310:265 ;
    skos:prefLabel "Item I266"@en-AU ;
    dcat:accessURL <https://www.legislation.gov.au/F2021L00310/2023-08-04/2023-08-04/text/1/epub/OEBPS/document_1/document_1.html#_Toc145601592> ;
    dcat:landingPage "https://www.legislation.gov.au/F2021L00310/2023-08-04/2023-08-04/text/1/epub/OEBPS/document_1/document_1.html#_Toc145601592"^^xsd:anyURI ;
    dcat:theme legcons:Item .

F2021L00310:268 a legcons:Item,
        owl:Class,
        dcat:Resource ;
    rdfs:label "Item - I268 12 2  Allocations of inspection services in effect immediately before commencement time"@en-AU ;
    dct:isPartOf F2021L00310:267 ;
    dct:isReferencedBy F2021L00310: ;
    rdfs:comment "12 2  Allocations of inspection services in effect immediately before commencement time - Abrievated Graph Key: I268"@en-AU ;
    skos:definition "12 2  Allocations of inspection services in effect immediately before commencement time"@en-AU ;
    skos:narrower F2021L00310:267 ;
    skos:prefLabel "Item I268"@en-AU ;
    dcat:accessURL <https://www.legislation.gov.au/F2021L00310/2023-08-04/2023-08-04/text/1/epub/OEBPS/document_1/document_1.html#_Toc145601594> ;
    dcat:landingPage "https://www.legislation.gov.au/F2021L00310/2023-08-04/2023-08-04/text/1/epub/OEBPS/document_1/document_1.html#_Toc145601594"^^xsd:anyURI ;
    dcat:theme legcons:Item .

F2021L00310:269 a legcons:Item,
        owl:Class,
        dcat:Resource ;
    rdfs:label "Item - I269 12 3  Application for inspection services not decided or notice of decision not given before commencement time"@en-AU ;
    dct:isPartOf F2021L00310:267 ;
    dct:isReferencedBy F2021L00310: ;
    rdfs:comment "12 3  Application for inspection services not decided or notice of decision not given before commencement time - Abrievated Graph Key: I269"@en-AU ;
    skos:definition "12 3  Application for inspection services not decided or notice of decision not given before commencement time"@en-AU ;
    skos:narrower F2021L00310:267 ;
    skos:prefLabel "Item I269"@en-AU ;
    dcat:accessURL <https://www.legislation.gov.au/F2021L00310/2023-08-04/2023-08-04/text/1/epub/OEBPS/document_1/document_1.html#_Toc145601595> ;
    dcat:landingPage "https://www.legislation.gov.au/F2021L00310/2023-08-04/2023-08-04/text/1/epub/OEBPS/document_1/document_1.html#_Toc145601595"^^xsd:anyURI ;
    dcat:theme legcons:Item .

F2021L00310:27 a legcons:Item,
        owl:Class,
        dcat:Resource ;
    rdfs:label "Item - I27 2 10  Revocation of exemptionmatter to which Secretary must have regard"@en-AU ;
    dct:isPartOf F2021L00310:21 ;
    dct:isReferencedBy F2021L00310: ;
    rdfs:comment "2 10  Revocation of exemptionmatter to which Secretary must have regard - Abrievated Graph Key: I27"@en-AU ;
    skos:definition "2 10  Revocation of exemptionmatter to which Secretary must have regard"@en-AU ;
    skos:narrower F2021L00310:21 ;
    skos:prefLabel "Item I27"@en-AU ;
    dcat:accessURL <https://www.legislation.gov.au/F2021L00310/2023-08-04/2023-08-04/text/1/epub/OEBPS/document_1/document_1.html#_Toc145601353> ;
    dcat:landingPage "https://www.legislation.gov.au/F2021L00310/2023-08-04/2023-08-04/text/1/epub/OEBPS/document_1/document_1.html#_Toc145601353"^^xsd:anyURI ;
    dcat:theme legcons:Item .

F2021L00310:270 a legcons:Item,
        owl:Class,
        dcat:Resource ;
    rdfs:label "Item - I270 12 4  Notice of preliminary determination of allocation given before commencement time"@en-AU ;
    dct:isPartOf F2021L00310:267 ;
    dct:isReferencedBy F2021L00310: ;
    rdfs:comment "12 4  Notice of preliminary determination of allocation given before commencement time - Abrievated Graph Key: I270"@en-AU ;
    skos:definition "12 4  Notice of preliminary determination of allocation given before commencement time"@en-AU ;
    skos:narrower F2021L00310:267 ;
    skos:prefLabel "Item I270"@en-AU ;
    dcat:accessURL <https://www.legislation.gov.au/F2021L00310/2023-08-04/2023-08-04/text/1/epub/OEBPS/document_1/document_1.html#_Toc145601596> ;
    dcat:landingPage "https://www.legislation.gov.au/F2021L00310/2023-08-04/2023-08-04/text/1/epub/OEBPS/document_1/document_1.html#_Toc145601596"^^xsd:anyURI ;
    dcat:theme legcons:Item .

F2021L00310:271 a legcons:Item,
        owl:Class,
        dcat:Resource ;
    rdfs:label "Item - I271 12 5  Preliminary determination of allocation agreed before commencement time"@en-AU ;
    dct:isPartOf F2021L00310:267 ;
    dct:isReferencedBy F2021L00310: ;
    rdfs:comment "12 5  Preliminary determination of allocation agreed before commencement time - Abrievated Graph Key: I271"@en-AU ;
    skos:definition "12 5  Preliminary determination of allocation agreed before commencement time"@en-AU ;
    skos:narrower F2021L00310:267 ;
    skos:prefLabel "Item I271"@en-AU ;
    dcat:accessURL <https://www.legislation.gov.au/F2021L00310/2023-08-04/2023-08-04/text/1/epub/OEBPS/document_1/document_1.html#_Toc145601597> ;
    dcat:landingPage "https://www.legislation.gov.au/F2021L00310/2023-08-04/2023-08-04/text/1/epub/OEBPS/document_1/document_1.html#_Toc145601597"^^xsd:anyURI ;
    dcat:theme legcons:Item .

F2021L00310:272 a legcons:Item,
        owl:Class,
        dcat:Resource ;
    rdfs:label "Item - I272 12 6  Revised determination made but notice not given before commencement time"@en-AU ;
    dct:isPartOf F2021L00310:267 ;
    dct:isReferencedBy F2021L00310: ;
    rdfs:comment "12 6  Revised determination made but notice not given before commencement time - Abrievated Graph Key: I272"@en-AU ;
    skos:definition "12 6  Revised determination made but notice not given before commencement time"@en-AU ;
    skos:narrower F2021L00310:267 ;
    skos:prefLabel "Item I272"@en-AU ;
    dcat:accessURL <https://www.legislation.gov.au/F2021L00310/2023-08-04/2023-08-04/text/1/epub/OEBPS/document_1/document_1.html#_Toc145601598> ;
    dcat:landingPage "https://www.legislation.gov.au/F2021L00310/2023-08-04/2023-08-04/text/1/epub/OEBPS/document_1/document_1.html#_Toc145601598"^^xsd:anyURI ;
    dcat:theme legcons:Item .

F2021L00310:273 a legcons:Item,
        owl:Class,
        dcat:Resource ;
    rdfs:label "Item - I273 12 7  Notice of revised determination of inspection services given before commencement time"@en-AU ;
    dct:isPartOf F2021L00310:267 ;
    dct:isReferencedBy F2021L00310: ;
    rdfs:comment "12 7  Notice of revised determination of inspection services given before commencement time - Abrievated Graph Key: I273"@en-AU ;
    skos:definition "12 7  Notice of revised determination of inspection services given before commencement time"@en-AU ;
    skos:narrower F2021L00310:267 ;
    skos:prefLabel "Item I273"@en-AU ;
    dcat:accessURL <https://www.legislation.gov.au/F2021L00310/2023-08-04/2023-08-04/text/1/epub/OEBPS/document_1/document_1.html#_Toc145601599> ;
    dcat:landingPage "https://www.legislation.gov.au/F2021L00310/2023-08-04/2023-08-04/text/1/epub/OEBPS/document_1/document_1.html#_Toc145601599"^^xsd:anyURI ;
    dcat:theme legcons:Item .

F2021L00310:274 a legcons:Item,
        owl:Class,
        dcat:Resource ;
    rdfs:label "Item - I274 12 8  Revised determination of allocation agreed before commencement time"@en-AU ;
    dct:isPartOf F2021L00310:267 ;
    dct:isReferencedBy F2021L00310: ;
    rdfs:comment "12 8  Revised determination of allocation agreed before commencement time - Abrievated Graph Key: I274"@en-AU ;
    skos:definition "12 8  Revised determination of allocation agreed before commencement time"@en-AU ;
    skos:narrower F2021L00310:267 ;
    skos:prefLabel "Item I274"@en-AU ;
    dcat:accessURL <https://www.legislation.gov.au/F2021L00310/2023-08-04/2023-08-04/text/1/epub/OEBPS/document_1/document_1.html#_Toc145601600> ;
    dcat:landingPage "https://www.legislation.gov.au/F2021L00310/2023-08-04/2023-08-04/text/1/epub/OEBPS/document_1/document_1.html#_Toc145601600"^^xsd:anyURI ;
    dcat:theme legcons:Item .

F2021L00310:275 a legcons:Item,
        owl:Class,
        dcat:Resource ;
    rdfs:label "Item - I275 12 9  Application for review committee made but committee not established before commencement time"@en-AU ;
    dct:isPartOf F2021L00310:267 ;
    dct:isReferencedBy F2021L00310: ;
    rdfs:comment "12 9  Application for review committee made but committee not established before commencement time - Abrievated Graph Key: I275"@en-AU ;
    skos:definition "12 9  Application for review committee made but committee not established before commencement time"@en-AU ;
    skos:narrower F2021L00310:267 ;
    skos:prefLabel "Item I275"@en-AU ;
    dcat:accessURL <https://www.legislation.gov.au/F2021L00310/2023-08-04/2023-08-04/text/1/epub/OEBPS/document_1/document_1.html#_Toc145601601> ;
    dcat:landingPage "https://www.legislation.gov.au/F2021L00310/2023-08-04/2023-08-04/text/1/epub/OEBPS/document_1/document_1.html#_Toc145601601"^^xsd:anyURI ;
    dcat:theme legcons:Item .

F2021L00310:276 a legcons:Item,
        owl:Class,
        dcat:Resource ;
    rdfs:label "Item - I276 12 10  Committee review in progress before commencement time"@en-AU ;
    dct:isPartOf F2021L00310:267 ;
    dct:isReferencedBy F2021L00310: ;
    rdfs:comment "12 10  Committee review in progress before commencement time - Abrievated Graph Key: I276"@en-AU ;
    skos:definition "12 10  Committee review in progress before commencement time"@en-AU ;
    skos:narrower F2021L00310:267 ;
    skos:prefLabel "Item I276"@en-AU ;
    dcat:accessURL <https://www.legislation.gov.au/F2021L00310/2023-08-04/2023-08-04/text/1/epub/OEBPS/document_1/document_1.html#_Toc145601602> ;
    dcat:landingPage "https://www.legislation.gov.au/F2021L00310/2023-08-04/2023-08-04/text/1/epub/OEBPS/document_1/document_1.html#_Toc145601602"^^xsd:anyURI ;
    dcat:theme legcons:Item .

F2021L00310:277 a legcons:Item,
        owl:Class,
        dcat:Resource ;
    rdfs:label "Item - I277 12 11  Determination reconsidered but notice not given before commencement time"@en-AU ;
    dct:isPartOf F2021L00310:267 ;
    dct:isReferencedBy F2021L00310: ;
    rdfs:comment "12 11  Determination reconsidered but notice not given before commencement time - Abrievated Graph Key: I277"@en-AU ;
    skos:definition "12 11  Determination reconsidered but notice not given before commencement time"@en-AU ;
    skos:narrower F2021L00310:267 ;
    skos:prefLabel "Item I277"@en-AU ;
    dcat:accessURL <https://www.legislation.gov.au/F2021L00310/2023-08-04/2023-08-04/text/1/epub/OEBPS/document_1/document_1.html#_Toc145601603> ;
    dcat:landingPage "https://www.legislation.gov.au/F2021L00310/2023-08-04/2023-08-04/text/1/epub/OEBPS/document_1/document_1.html#_Toc145601603"^^xsd:anyURI ;
    dcat:theme legcons:Item .

F2021L00310:278 a legcons:Item,
        owl:Class,
        dcat:Resource ;
    rdfs:label "Item - I278 12 12  Application to alter inspection services not decided before commencement time"@en-AU ;
    dct:isPartOf F2021L00310:267 ;
    dct:isReferencedBy F2021L00310: ;
    rdfs:comment "12 12  Application to alter inspection services not decided before commencement time - Abrievated Graph Key: I278"@en-AU ;
    skos:definition "12 12  Application to alter inspection services not decided before commencement time"@en-AU ;
    skos:narrower F2021L00310:267 ;
    skos:prefLabel "Item I278"@en-AU ;
    dcat:accessURL <https://www.legislation.gov.au/F2021L00310/2023-08-04/2023-08-04/text/1/epub/OEBPS/document_1/document_1.html#_Toc145601604> ;
    dcat:landingPage "https://www.legislation.gov.au/F2021L00310/2023-08-04/2023-08-04/text/1/epub/OEBPS/document_1/document_1.html#_Toc145601604"^^xsd:anyURI ;
    dcat:theme legcons:Item .

F2021L00310:279 a legcons:Item,
        owl:Class,
        dcat:Resource ;
    rdfs:label "Item - I279 12 13  Application for additional inspection services not decided before commencement time"@en-AU ;
    dct:isPartOf F2021L00310:267 ;
    dct:isReferencedBy F2021L00310: ;
    rdfs:comment "12 13  Application for additional inspection services not decided before commencement time - Abrievated Graph Key: I279"@en-AU ;
    skos:definition "12 13  Application for additional inspection services not decided before commencement time"@en-AU ;
    skos:narrower F2021L00310:267 ;
    skos:prefLabel "Item I279"@en-AU ;
    dcat:accessURL <https://www.legislation.gov.au/F2021L00310/2023-08-04/2023-08-04/text/1/epub/OEBPS/document_1/document_1.html#_Toc145601605> ;
    dcat:landingPage "https://www.legislation.gov.au/F2021L00310/2023-08-04/2023-08-04/text/1/epub/OEBPS/document_1/document_1.html#_Toc145601605"^^xsd:anyURI ;
    dcat:theme legcons:Item .

F2021L00310:280 a legcons:Item,
        owl:Class,
        dcat:Resource ;
    rdfs:label "Item - I280 12 14  Notice of termination of additional inspection services given before commencement time"@en-AU ;
    dct:isPartOf F2021L00310:267 ;
    dct:isReferencedBy F2021L00310: ;
    rdfs:comment "12 14  Notice of termination of additional inspection services given before commencement time - Abrievated Graph Key: I280"@en-AU ;
    skos:definition "12 14  Notice of termination of additional inspection services given before commencement time"@en-AU ;
    skos:narrower F2021L00310:267 ;
    skos:prefLabel "Item I280"@en-AU ;
    dcat:accessURL <https://www.legislation.gov.au/F2021L00310/2023-08-04/2023-08-04/text/1/epub/OEBPS/document_1/document_1.html#_Toc145601606> ;
    dcat:landingPage "https://www.legislation.gov.au/F2021L00310/2023-08-04/2023-08-04/text/1/epub/OEBPS/document_1/document_1.html#_Toc145601606"^^xsd:anyURI ;
    dcat:theme legcons:Item .

F2021L00310:281 a legcons:Item,
        owl:Class,
        dcat:Resource ;
    rdfs:label "Item - I281 12 15  Notice of shutdown given before commencement time"@en-AU ;
    dct:isPartOf F2021L00310:267 ;
    dct:isReferencedBy F2021L00310: ;
    rdfs:comment "12 15  Notice of shutdown given before commencement time - Abrievated Graph Key: I281"@en-AU ;
    skos:definition "12 15  Notice of shutdown given before commencement time"@en-AU ;
    skos:narrower F2021L00310:267 ;
    skos:prefLabel "Item I281"@en-AU ;
    dcat:accessURL <https://www.legislation.gov.au/F2021L00310/2023-08-04/2023-08-04/text/1/epub/OEBPS/document_1/document_1.html#_Toc145601607> ;
    dcat:landingPage "https://www.legislation.gov.au/F2021L00310/2023-08-04/2023-08-04/text/1/epub/OEBPS/document_1/document_1.html#_Toc145601607"^^xsd:anyURI ;
    dcat:theme legcons:Item .

F2021L00310:282 a legcons:Item,
        owl:Class,
        dcat:Resource ;
    rdfs:label "Item - I282 12 16  Variation of allocation for change of circumstance not advised before commencement time"@en-AU ;
    dct:isPartOf F2021L00310:267 ;
    dct:isReferencedBy F2021L00310: ;
    rdfs:comment "12 16  Variation of allocation for change of circumstance not advised before commencement time - Abrievated Graph Key: I282"@en-AU ;
    skos:definition "12 16  Variation of allocation for change of circumstance not advised before commencement time"@en-AU ;
    skos:narrower F2021L00310:267 ;
    skos:prefLabel "Item I282"@en-AU ;
    dcat:accessURL <https://www.legislation.gov.au/F2021L00310/2023-08-04/2023-08-04/text/1/epub/OEBPS/document_1/document_1.html#_Toc145601608> ;
    dcat:landingPage "https://www.legislation.gov.au/F2021L00310/2023-08-04/2023-08-04/text/1/epub/OEBPS/document_1/document_1.html#_Toc145601608"^^xsd:anyURI ;
    dcat:theme legcons:Item .

F2021L00310:283 a legcons:Item,
        owl:Class,
        dcat:Resource ;
    rdfs:label "Item - I283 12 17  Disputed allocation not decided before commencement time"@en-AU ;
    dct:isPartOf F2021L00310:267 ;
    dct:isReferencedBy F2021L00310: ;
    rdfs:comment "12 17  Disputed allocation not decided before commencement time - Abrievated Graph Key: I283"@en-AU ;
    skos:definition "12 17  Disputed allocation not decided before commencement time"@en-AU ;
    skos:narrower F2021L00310:267 ;
    skos:prefLabel "Item I283"@en-AU ;
    dcat:accessURL <https://www.legislation.gov.au/F2021L00310/2023-08-04/2023-08-04/text/1/epub/OEBPS/document_1/document_1.html#_Toc145601609> ;
    dcat:landingPage "https://www.legislation.gov.au/F2021L00310/2023-08-04/2023-08-04/text/1/epub/OEBPS/document_1/document_1.html#_Toc145601609"^^xsd:anyURI ;
    dcat:theme legcons:Item .

F2021L00310:284 a legcons:Item,
        owl:Class,
        dcat:Resource ;
    rdfs:label "Item - I284 12 18  Notice of reconsideration of disputed allocation not given before commencement time"@en-AU ;
    dct:isPartOf F2021L00310:267 ;
    dct:isReferencedBy F2021L00310: ;
    rdfs:comment "12 18  Notice of reconsideration of disputed allocation not given before commencement time - Abrievated Graph Key: I284"@en-AU ;
    skos:definition "12 18  Notice of reconsideration of disputed allocation not given before commencement time"@en-AU ;
    skos:narrower F2021L00310:267 ;
    skos:prefLabel "Item I284"@en-AU ;
    dcat:accessURL <https://www.legislation.gov.au/F2021L00310/2023-08-04/2023-08-04/text/1/epub/OEBPS/document_1/document_1.html#_Toc145601610> ;
    dcat:landingPage "https://www.legislation.gov.au/F2021L00310/2023-08-04/2023-08-04/text/1/epub/OEBPS/document_1/document_1.html#_Toc145601610"^^xsd:anyURI ;
    dcat:theme legcons:Item .

F2021L00310:286 a legcons:Item,
        owl:Class,
        dcat:Resource ;
    rdfs:label "Item - I286 12 19  Information and declarations given before commencement time"@en-AU ;
    dct:isPartOf F2021L00310:285 ;
    dct:isReferencedBy F2021L00310: ;
    rdfs:comment "12 19  Information and declarations given before commencement time - Abrievated Graph Key: I286"@en-AU ;
    skos:definition "12 19  Information and declarations given before commencement time"@en-AU ;
    skos:narrower F2021L00310:285 ;
    skos:prefLabel "Item I286"@en-AU ;
    dcat:accessURL <https://www.legislation.gov.au/F2021L00310/2023-08-04/2023-08-04/text/1/epub/OEBPS/document_1/document_1.html#_Toc145601612> ;
    dcat:landingPage "https://www.legislation.gov.au/F2021L00310/2023-08-04/2023-08-04/text/1/epub/OEBPS/document_1/document_1.html#_Toc145601612"^^xsd:anyURI ;
    dcat:theme legcons:Item .

F2021L00310:289 a legcons:Item,
        owl:Class,
        dcat:Resource ;
    rdfs:label "Item - I289 12 20  Request for translation not complied with before commencement time"@en-AU ;
    dct:isPartOf F2021L00310:288 ;
    dct:isReferencedBy F2021L00310: ;
    rdfs:comment "12 20  Request for translation not complied with before commencement time - Abrievated Graph Key: I289"@en-AU ;
    skos:definition "12 20  Request for translation not complied with before commencement time"@en-AU ;
    skos:narrower F2021L00310:288 ;
    skos:prefLabel "Item I289"@en-AU ;
    dcat:accessURL <https://www.legislation.gov.au/F2021L00310/2023-08-04/2023-08-04/text/1/epub/OEBPS/document_1/document_1.html#_Toc145601615> ;
    dcat:landingPage "https://www.legislation.gov.au/F2021L00310/2023-08-04/2023-08-04/text/1/epub/OEBPS/document_1/document_1.html#_Toc145601615"^^xsd:anyURI ;
    dcat:theme legcons:Item .

F2021L00310:29 a legcons:Item,
        owl:Class,
        dcat:Resource ;
    rdfs:label "Item - I29 2 11  When government certificate may be issued in relation to poultry meat or poultry meat products"@en-AU ;
    dct:isPartOf F2021L00310:28 ;
    dct:isReferencedBy F2021L00310: ;
    rdfs:comment "2 11  When government certificate may be issued in relation to poultry meat or poultry meat products - Abrievated Graph Key: I29"@en-AU ;
    skos:definition "2 11  When government certificate may be issued in relation to poultry meat or poultry meat products"@en-AU ;
    skos:narrower F2021L00310:28 ;
    skos:prefLabel "Item I29"@en-AU ;
    dcat:accessURL <https://www.legislation.gov.au/F2021L00310/2023-08-04/2023-08-04/text/1/epub/OEBPS/document_1/document_1.html#_Toc145601355> ;
    dcat:landingPage "https://www.legislation.gov.au/F2021L00310/2023-08-04/2023-08-04/text/1/epub/OEBPS/document_1/document_1.html#_Toc145601355"^^xsd:anyURI ;
    dcat:theme legcons:Item .

F2021L00310:291 a legcons:Item,
        owl:Class,
        dcat:Resource ;
    rdfs:label "Item - I291 12 21  Person approved before commencement time to manufacture an official mark"@en-AU ;
    dct:isPartOf F2021L00310:290 ;
    dct:isReferencedBy F2021L00310: ;
    rdfs:comment "12 21  Person approved before commencement time to manufacture an official mark - Abrievated Graph Key: I291"@en-AU ;
    skos:definition "12 21  Person approved before commencement time to manufacture an official mark"@en-AU ;
    skos:narrower F2021L00310:290 ;
    skos:prefLabel "Item I291"@en-AU ;
    dcat:accessURL <https://www.legislation.gov.au/F2021L00310/2023-08-04/2023-08-04/text/1/epub/OEBPS/document_1/document_1.html#_Toc145601617> ;
    dcat:landingPage "https://www.legislation.gov.au/F2021L00310/2023-08-04/2023-08-04/text/1/epub/OEBPS/document_1/document_1.html#_Toc145601617"^^xsd:anyURI ;
    dcat:theme legcons:Item .

F2021L00310:292 a legcons:Item,
        owl:Class,
        dcat:Resource ;
    rdfs:label "Item - I292 12 22  Person approved before commencement time to apply an official mark"@en-AU ;
    dct:isPartOf F2021L00310:290 ;
    dct:isReferencedBy F2021L00310: ;
    rdfs:comment "12 22  Person approved before commencement time to apply an official mark - Abrievated Graph Key: I292"@en-AU ;
    skos:definition "12 22  Person approved before commencement time to apply an official mark"@en-AU ;
    skos:narrower F2021L00310:290 ;
    skos:prefLabel "Item I292"@en-AU ;
    dcat:accessURL <https://www.legislation.gov.au/F2021L00310/2023-08-04/2023-08-04/text/1/epub/OEBPS/document_1/document_1.html#_Toc145601618> ;
    dcat:landingPage "https://www.legislation.gov.au/F2021L00310/2023-08-04/2023-08-04/text/1/epub/OEBPS/document_1/document_1.html#_Toc145601618"^^xsd:anyURI ;
    dcat:theme legcons:Item .

F2021L00310:294 a legcons:Item,
        owl:Class,
        dcat:Resource ;
    rdfs:label "Item - I294 12 23  Person approved before commencement time to manufacture an official marking device"@en-AU ;
    dct:isPartOf F2021L00310:293 ;
    dct:isReferencedBy F2021L00310: ;
    rdfs:comment "12 23  Person approved before commencement time to manufacture an official marking device - Abrievated Graph Key: I294"@en-AU ;
    skos:definition "12 23  Person approved before commencement time to manufacture an official marking device"@en-AU ;
    skos:narrower F2021L00310:293 ;
    skos:prefLabel "Item I294"@en-AU ;
    dcat:accessURL <https://www.legislation.gov.au/F2021L00310/2023-08-04/2023-08-04/text/1/epub/OEBPS/document_1/document_1.html#_Toc145601620> ;
    dcat:landingPage "https://www.legislation.gov.au/F2021L00310/2023-08-04/2023-08-04/text/1/epub/OEBPS/document_1/document_1.html#_Toc145601620"^^xsd:anyURI ;
    dcat:theme legcons:Item .

F2021L00310:295 a legcons:Item,
        owl:Class,
        dcat:Resource ;
    rdfs:label "Item - I295 12 24  Person approved before commencement time to possess an official marking device"@en-AU ;
    dct:isPartOf F2021L00310:293 ;
    dct:isReferencedBy F2021L00310: ;
    rdfs:comment "12 24  Person approved before commencement time to possess an official marking device - Abrievated Graph Key: I295"@en-AU ;
    skos:definition "12 24  Person approved before commencement time to possess an official marking device"@en-AU ;
    skos:narrower F2021L00310:293 ;
    skos:prefLabel "Item I295"@en-AU ;
    dcat:accessURL <https://www.legislation.gov.au/F2021L00310/2023-08-04/2023-08-04/text/1/epub/OEBPS/document_1/document_1.html#_Toc145601621> ;
    dcat:landingPage "https://www.legislation.gov.au/F2021L00310/2023-08-04/2023-08-04/text/1/epub/OEBPS/document_1/document_1.html#_Toc145601621"^^xsd:anyURI ;
    dcat:theme legcons:Item .

F2021L00310:298 a legcons:Item,
        owl:Class,
        dcat:Resource ;
    rdfs:label "Item - I298 12 25  Application for approval as auditor not decided or notice of decision not given before commencement time"@en-AU ;
    dct:isPartOf F2021L00310:297 ;
    dct:isReferencedBy F2021L00310: ;
    rdfs:comment "12 25  Application for approval as auditor not decided or notice of decision not given before commencement time - Abrievated Graph Key: I298"@en-AU ;
    skos:definition "12 25  Application for approval as auditor not decided or notice of decision not given before commencement time"@en-AU ;
    skos:narrower F2021L00310:297 ;
    skos:prefLabel "Item I298"@en-AU ;
    dcat:accessURL <https://www.legislation.gov.au/F2021L00310/2023-08-04/2023-08-04/text/1/epub/OEBPS/document_1/document_1.html#_Toc145601624> ;
    dcat:landingPage "https://www.legislation.gov.au/F2021L00310/2023-08-04/2023-08-04/text/1/epub/OEBPS/document_1/document_1.html#_Toc145601624"^^xsd:anyURI ;
    dcat:theme legcons:Item .

F2021L00310:299 a legcons:Item,
        owl:Class,
        dcat:Resource ;
    rdfs:label "Item - I299 12 26  Request for further information not complied with before commencement time"@en-AU ;
    dct:isPartOf F2021L00310:297 ;
    dct:isReferencedBy F2021L00310: ;
    rdfs:comment "12 26  Request for further information not complied with before commencement time - Abrievated Graph Key: I299"@en-AU ;
    skos:definition "12 26  Request for further information not complied with before commencement time"@en-AU ;
    skos:narrower F2021L00310:297 ;
    skos:prefLabel "Item I299"@en-AU ;
    dcat:accessURL <https://www.legislation.gov.au/F2021L00310/2023-08-04/2023-08-04/text/1/epub/OEBPS/document_1/document_1.html#_Toc145601625> ;
    dcat:landingPage "https://www.legislation.gov.au/F2021L00310/2023-08-04/2023-08-04/text/1/epub/OEBPS/document_1/document_1.html#_Toc145601625"^^xsd:anyURI ;
    dcat:theme legcons:Item .

F2021L00310:3 a legcons:Item,
        owl:Class,
        dcat:Resource ;
    rdfs:label "Item - I3 1 1  Name"@en-AU ;
    dct:isPartOf F2021L00310:1 ;
    dct:isReferencedBy F2021L00310: ;
    rdfs:comment "1 1  Name - Abrievated Graph Key: I3"@en-AU ;
    skos:definition "1 1  Name"@en-AU ;
    skos:narrower F2021L00310:1 ;
    skos:prefLabel "Item I3"@en-AU ;
    dcat:accessURL <https://www.legislation.gov.au/F2021L00310/2023-08-04/2023-08-04/text/1/epub/OEBPS/document_1/document_1.html#_Toc145601329> ;
    dcat:landingPage "https://www.legislation.gov.au/F2021L00310/2023-08-04/2023-08-04/text/1/epub/OEBPS/document_1/document_1.html#_Toc145601329"^^xsd:anyURI ;
    dcat:theme legcons:Item .

F2021L00310:30 a legcons:Item,
        owl:Class,
        dcat:Resource ;
    rdfs:label "Item - I30 2 12  Declaration to accompany application for government certificate"@en-AU ;
    dct:isPartOf F2021L00310:28 ;
    dct:isReferencedBy F2021L00310: ;
    rdfs:comment "2 12  Declaration to accompany application for government certificate - Abrievated Graph Key: I30"@en-AU ;
    skos:definition "2 12  Declaration to accompany application for government certificate"@en-AU ;
    skos:narrower F2021L00310:28 ;
    skos:prefLabel "Item I30"@en-AU ;
    dcat:accessURL <https://www.legislation.gov.au/F2021L00310/2023-08-04/2023-08-04/text/1/epub/OEBPS/document_1/document_1.html#_Toc145601356> ;
    dcat:landingPage "https://www.legislation.gov.au/F2021L00310/2023-08-04/2023-08-04/text/1/epub/OEBPS/document_1/document_1.html#_Toc145601356"^^xsd:anyURI ;
    dcat:theme legcons:Item .

F2021L00310:300 a legcons:Item,
        owl:Class,
        dcat:Resource ;
    rdfs:label "Item - I300 12 27  Decision to revoke approval as auditor decided but notice not given before commencement time"@en-AU ;
    dct:isPartOf F2021L00310:297 ;
    dct:isReferencedBy F2021L00310: ;
    rdfs:comment "12 27  Decision to revoke approval as auditor decided but notice not given before commencement time - Abrievated Graph Key: I300"@en-AU ;
    skos:definition "12 27  Decision to revoke approval as auditor decided but notice not given before commencement time"@en-AU ;
    skos:narrower F2021L00310:297 ;
    skos:prefLabel "Item I300"@en-AU ;
    dcat:accessURL <https://www.legislation.gov.au/F2021L00310/2023-08-04/2023-08-04/text/1/epub/OEBPS/document_1/document_1.html#_Toc145601626> ;
    dcat:landingPage "https://www.legislation.gov.au/F2021L00310/2023-08-04/2023-08-04/text/1/epub/OEBPS/document_1/document_1.html#_Toc145601626"^^xsd:anyURI ;
    dcat:theme legcons:Item .

F2021L00310:302 a legcons:Item,
        owl:Class,
        dcat:Resource ;
    rdfs:label "Item - I302 12 28  Decision or disposition applied but not complied with before commencement time"@en-AU ;
    dct:isPartOf F2021L00310:301 ;
    dct:isReferencedBy F2021L00310: ;
    rdfs:comment "12 28  Decision or disposition applied but not complied with before commencement time - Abrievated Graph Key: I302"@en-AU ;
    skos:definition "12 28  Decision or disposition applied but not complied with before commencement time"@en-AU ;
    skos:narrower F2021L00310:301 ;
    skos:prefLabel "Item I302"@en-AU ;
    dcat:accessURL <https://www.legislation.gov.au/F2021L00310/2023-08-04/2023-08-04/text/1/epub/OEBPS/document_1/document_1.html#_Toc145601628> ;
    dcat:landingPage "https://www.legislation.gov.au/F2021L00310/2023-08-04/2023-08-04/text/1/epub/OEBPS/document_1/document_1.html#_Toc145601628"^^xsd:anyURI ;
    dcat:theme legcons:Item .

F2021L00310:303 a legcons:Item,
        owl:Class,
        dcat:Resource ;
    rdfs:label "Item - I303 12 29  Certificate of condemnation requested but not given before commencement time"@en-AU ;
    dct:isPartOf F2021L00310:301 ;
    dct:isReferencedBy F2021L00310: ;
    rdfs:comment "12 29  Certificate of condemnation requested but not given before commencement time - Abrievated Graph Key: I303"@en-AU ;
    skos:definition "12 29  Certificate of condemnation requested but not given before commencement time"@en-AU ;
    skos:narrower F2021L00310:301 ;
    skos:prefLabel "Item I303"@en-AU ;
    dcat:accessURL <https://www.legislation.gov.au/F2021L00310/2023-08-04/2023-08-04/text/1/epub/OEBPS/document_1/document_1.html#_Toc145601629> ;
    dcat:landingPage "https://www.legislation.gov.au/F2021L00310/2023-08-04/2023-08-04/text/1/epub/OEBPS/document_1/document_1.html#_Toc145601629"^^xsd:anyURI ;
    dcat:theme legcons:Item .

F2021L00310:305 a legcons:Item,
        owl:Class,
        dcat:Resource ;
    rdfs:label "Item - I305 Endnote 1 About the endnotes"@en-AU ;
    dct:isPartOf F2021L00310:304 ;
    dct:isReferencedBy F2021L00310: ;
    rdfs:comment "Endnote 1 About the endnotes - Abrievated Graph Key: I305"@en-AU ;
    skos:definition "Endnote 1 About the endnotes"@en-AU ;
    skos:narrower F2021L00310:304 ;
    skos:prefLabel "Item I305"@en-AU ;
    dcat:accessURL <https://www.legislation.gov.au/F2021L00310/2023-08-04/2023-08-04/text/1/epub/OEBPS/document_1/document_1.html#_Toc145601631> ;
    dcat:landingPage "https://www.legislation.gov.au/F2021L00310/2023-08-04/2023-08-04/text/1/epub/OEBPS/document_1/document_1.html#_Toc145601631"^^xsd:anyURI ;
    dcat:theme legcons:Item .

F2021L00310:306 a legcons:Item,
        owl:Class,
        dcat:Resource ;
    rdfs:label "Item - I306 Endnote 2 Abbreviation key"@en-AU ;
    dct:isPartOf F2021L00310:304 ;
    dct:isReferencedBy F2021L00310: ;
    rdfs:comment "Endnote 2 Abbreviation key - Abrievated Graph Key: I306"@en-AU ;
    skos:definition "Endnote 2 Abbreviation key"@en-AU ;
    skos:narrower F2021L00310:304 ;
    skos:prefLabel "Item I306"@en-AU ;
    dcat:accessURL <https://www.legislation.gov.au/F2021L00310/2023-08-04/2023-08-04/text/1/epub/OEBPS/document_1/document_1.html#_Toc145601632> ;
    dcat:landingPage "https://www.legislation.gov.au/F2021L00310/2023-08-04/2023-08-04/text/1/epub/OEBPS/document_1/document_1.html#_Toc145601632"^^xsd:anyURI ;
    dcat:theme legcons:Item .

F2021L00310:307 a legcons:Item,
        owl:Class,
        dcat:Resource ;
    rdfs:label "Item - I307 Endnote 3 Legislation history"@en-AU ;
    dct:isPartOf F2021L00310:304 ;
    dct:isReferencedBy F2021L00310: ;
    rdfs:comment "Endnote 3 Legislation history - Abrievated Graph Key: I307"@en-AU ;
    skos:definition "Endnote 3 Legislation history"@en-AU ;
    skos:narrower F2021L00310:304 ;
    skos:prefLabel "Item I307"@en-AU ;
    dcat:accessURL <https://www.legislation.gov.au/F2021L00310/2023-08-04/2023-08-04/text/1/epub/OEBPS/document_1/document_1.html#_Toc145601633> ;
    dcat:landingPage "https://www.legislation.gov.au/F2021L00310/2023-08-04/2023-08-04/text/1/epub/OEBPS/document_1/document_1.html#_Toc145601633"^^xsd:anyURI ;
    dcat:theme legcons:Item .

F2021L00310:308 a legcons:Item,
        owl:Class,
        dcat:Resource ;
    rdfs:label "Item - I308 Endnote 4 Amendment history"@en-AU ;
    dct:isPartOf F2021L00310:304 ;
    dct:isReferencedBy F2021L00310: ;
    rdfs:comment "Endnote 4 Amendment history - Abrievated Graph Key: I308"@en-AU ;
    skos:definition "Endnote 4 Amendment history"@en-AU ;
    skos:narrower F2021L00310:304 ;
    skos:prefLabel "Item I308"@en-AU ;
    dcat:accessURL <https://www.legislation.gov.au/F2021L00310/2023-08-04/2023-08-04/text/1/epub/OEBPS/document_1/document_1.html#_Toc145601634> ;
    dcat:landingPage "https://www.legislation.gov.au/F2021L00310/2023-08-04/2023-08-04/text/1/epub/OEBPS/document_1/document_1.html#_Toc145601634"^^xsd:anyURI ;
    dcat:theme legcons:Item .

F2021L00310:31 a legcons:Item,
        owl:Class,
        dcat:Resource ;
    rdfs:label "Item - I31 2 13  Circumstances for refusing to issue government certificate"@en-AU ;
    dct:isPartOf F2021L00310:28 ;
    dct:isReferencedBy F2021L00310: ;
    rdfs:comment "2 13  Circumstances for refusing to issue government certificate - Abrievated Graph Key: I31"@en-AU ;
    skos:definition "2 13  Circumstances for refusing to issue government certificate"@en-AU ;
    skos:narrower F2021L00310:28 ;
    skos:prefLabel "Item I31"@en-AU ;
    dcat:accessURL <https://www.legislation.gov.au/F2021L00310/2023-08-04/2023-08-04/text/1/epub/OEBPS/document_1/document_1.html#_Toc145601357> ;
    dcat:landingPage "https://www.legislation.gov.au/F2021L00310/2023-08-04/2023-08-04/text/1/epub/OEBPS/document_1/document_1.html#_Toc145601357"^^xsd:anyURI ;
    dcat:theme legcons:Item .

F2021L00310:32 a legcons:Item,
        owl:Class,
        dcat:Resource ;
    rdfs:label "Item - I32 2 14  Changes that require holder of certificate to give additional or corrected information to the issuing body"@en-AU ;
    dct:isPartOf F2021L00310:28 ;
    dct:isReferencedBy F2021L00310: ;
    rdfs:comment "2 14  Changes that require holder of certificate to give additional or corrected information to the issuing body - Abrievated Graph Key: I32"@en-AU ;
    skos:definition "2 14  Changes that require holder of certificate to give additional or corrected information to the issuing body"@en-AU ;
    skos:narrower F2021L00310:28 ;
    skos:prefLabel "Item I32"@en-AU ;
    dcat:accessURL <https://www.legislation.gov.au/F2021L00310/2023-08-04/2023-08-04/text/1/epub/OEBPS/document_1/document_1.html#_Toc145601358> ;
    dcat:landingPage "https://www.legislation.gov.au/F2021L00310/2023-08-04/2023-08-04/text/1/epub/OEBPS/document_1/document_1.html#_Toc145601358"^^xsd:anyURI ;
    dcat:theme legcons:Item .

F2021L00310:33 a legcons:Item,
        owl:Class,
        dcat:Resource ;
    rdfs:label "Item - I33 2 15  Return of government certificate"@en-AU ;
    dct:isPartOf F2021L00310:28 ;
    dct:isReferencedBy F2021L00310: ;
    rdfs:comment "2 15  Return of government certificate - Abrievated Graph Key: I33"@en-AU ;
    skos:definition "2 15  Return of government certificate"@en-AU ;
    skos:narrower F2021L00310:28 ;
    skos:prefLabel "Item I33"@en-AU ;
    dcat:accessURL <https://www.legislation.gov.au/F2021L00310/2023-08-04/2023-08-04/text/1/epub/OEBPS/document_1/document_1.html#_Toc145601359> ;
    dcat:landingPage "https://www.legislation.gov.au/F2021L00310/2023-08-04/2023-08-04/text/1/epub/OEBPS/document_1/document_1.html#_Toc145601359"^^xsd:anyURI ;
    dcat:theme legcons:Item .

F2021L00310:36 a legcons:Item,
        owl:Class,
        dcat:Resource ;
    rdfs:label "Item - I36 4 1  Purpose of this Part"@en-AU ;
    dct:isPartOf F2021L00310:35 ;
    dct:isReferencedBy F2021L00310: ;
    rdfs:comment "4 1  Purpose of this Part - Abrievated Graph Key: I36"@en-AU ;
    skos:definition "4 1  Purpose of this Part"@en-AU ;
    skos:narrower F2021L00310:35 ;
    skos:prefLabel "Item I36"@en-AU ;
    dcat:accessURL <https://www.legislation.gov.au/F2021L00310/2023-08-04/2023-08-04/text/1/epub/OEBPS/document_1/document_1.html#_Toc145601362> ;
    dcat:landingPage "https://www.legislation.gov.au/F2021L00310/2023-08-04/2023-08-04/text/1/epub/OEBPS/document_1/document_1.html#_Toc145601362"^^xsd:anyURI ;
    dcat:theme legcons:Item .

F2021L00310:37 a legcons:Item,
        owl:Class,
        dcat:Resource ;
    rdfs:label "Item - I37 4 2  Operations must be carried out in a way that will ensure requirements of the Act are complied with"@en-AU ;
    dct:isPartOf F2021L00310:35 ;
    dct:isReferencedBy F2021L00310: ;
    rdfs:comment "4 2  Operations must be carried out in a way that will ensure requirements of the Act are complied with - Abrievated Graph Key: I37"@en-AU ;
    skos:definition "4 2  Operations must be carried out in a way that will ensure requirements of the Act are complied with"@en-AU ;
    skos:narrower F2021L00310:35 ;
    skos:prefLabel "Item I37"@en-AU ;
    dcat:accessURL <https://www.legislation.gov.au/F2021L00310/2023-08-04/2023-08-04/text/1/epub/OEBPS/document_1/document_1.html#_Toc145601363> ;
    dcat:landingPage "https://www.legislation.gov.au/F2021L00310/2023-08-04/2023-08-04/text/1/epub/OEBPS/document_1/document_1.html#_Toc145601363"^^xsd:anyURI ;
    dcat:theme legcons:Item .

F2021L00310:38 a legcons:Item,
        owl:Class,
        dcat:Resource ;
    rdfs:label "Item - I38 4 3  Requirements of Australian Poultry Meat Standard must be met"@en-AU ;
    dct:isPartOf F2021L00310:35 ;
    dct:isReferencedBy F2021L00310: ;
    rdfs:comment "4 3  Requirements of Australian Poultry Meat Standard must be met - Abrievated Graph Key: I38"@en-AU ;
    skos:definition "4 3  Requirements of Australian Poultry Meat Standard must be met"@en-AU ;
    skos:narrower F2021L00310:35 ;
    skos:prefLabel "Item I38"@en-AU ;
    dcat:accessURL <https://www.legislation.gov.au/F2021L00310/2023-08-04/2023-08-04/text/1/epub/OEBPS/document_1/document_1.html#_Toc145601364> ;
    dcat:landingPage "https://www.legislation.gov.au/F2021L00310/2023-08-04/2023-08-04/text/1/epub/OEBPS/document_1/document_1.html#_Toc145601364"^^xsd:anyURI ;
    dcat:theme legcons:Item .

F2021L00310:39 a legcons:Item,
        owl:Class,
        dcat:Resource ;
    rdfs:label "Item - I39 4 4  Equipment facilities and essential services"@en-AU ;
    dct:isPartOf F2021L00310:35 ;
    dct:isReferencedBy F2021L00310: ;
    rdfs:comment "4 4  Equipment facilities and essential services - Abrievated Graph Key: I39"@en-AU ;
    skos:definition "4 4  Equipment facilities and essential services"@en-AU ;
    skos:narrower F2021L00310:35 ;
    skos:prefLabel "Item I39"@en-AU ;
    dcat:accessURL <https://www.legislation.gov.au/F2021L00310/2023-08-04/2023-08-04/text/1/epub/OEBPS/document_1/document_1.html#_Toc145601365> ;
    dcat:landingPage "https://www.legislation.gov.au/F2021L00310/2023-08-04/2023-08-04/text/1/epub/OEBPS/document_1/document_1.html#_Toc145601365"^^xsd:anyURI ;
    dcat:theme legcons:Item .

F2021L00310:4 a legcons:Item,
        owl:Class,
        dcat:Resource ;
    rdfs:label "Item - I4 1 3  Authority"@en-AU ;
    dct:isPartOf F2021L00310:1 ;
    dct:isReferencedBy F2021L00310: ;
    rdfs:comment "1 3  Authority - Abrievated Graph Key: I4"@en-AU ;
    skos:definition "1 3  Authority"@en-AU ;
    skos:narrower F2021L00310:1 ;
    skos:prefLabel "Item I4"@en-AU ;
    dcat:accessURL <https://www.legislation.gov.au/F2021L00310/2023-08-04/2023-08-04/text/1/epub/OEBPS/document_1/document_1.html#_Toc145601330> ;
    dcat:landingPage "https://www.legislation.gov.au/F2021L00310/2023-08-04/2023-08-04/text/1/epub/OEBPS/document_1/document_1.html#_Toc145601330"^^xsd:anyURI ;
    dcat:theme legcons:Item .

F2021L00310:40 a legcons:Item,
        owl:Class,
        dcat:Resource ;
    rdfs:label "Item - I40 4 5  Areas where post mortem inspections are carried out"@en-AU ;
    dct:isPartOf F2021L00310:35 ;
    dct:isReferencedBy F2021L00310: ;
    rdfs:comment "4 5  Areas where post mortem inspections are carried out - Abrievated Graph Key: I40"@en-AU ;
    skos:definition "4 5  Areas where post mortem inspections are carried out"@en-AU ;
    skos:narrower F2021L00310:35 ;
    skos:prefLabel "Item I40"@en-AU ;
    dcat:accessURL <https://www.legislation.gov.au/F2021L00310/2023-08-04/2023-08-04/text/1/epub/OEBPS/document_1/document_1.html#_Toc145601366> ;
    dcat:landingPage "https://www.legislation.gov.au/F2021L00310/2023-08-04/2023-08-04/text/1/epub/OEBPS/document_1/document_1.html#_Toc145601366"^^xsd:anyURI ;
    dcat:theme legcons:Item .

F2021L00310:41 a legcons:Item,
        owl:Class,
        dcat:Resource ;
    rdfs:label "Item - I41 4 6  Meat examination facility"@en-AU ;
    dct:isPartOf F2021L00310:35 ;
    dct:isReferencedBy F2021L00310: ;
    rdfs:comment "4 6  Meat examination facility - Abrievated Graph Key: I41"@en-AU ;
    skos:definition "4 6  Meat examination facility"@en-AU ;
    skos:narrower F2021L00310:35 ;
    skos:prefLabel "Item I41"@en-AU ;
    dcat:accessURL <https://www.legislation.gov.au/F2021L00310/2023-08-04/2023-08-04/text/1/epub/OEBPS/document_1/document_1.html#_Toc145601367> ;
    dcat:landingPage "https://www.legislation.gov.au/F2021L00310/2023-08-04/2023-08-04/text/1/epub/OEBPS/document_1/document_1.html#_Toc145601367"^^xsd:anyURI ;
    dcat:theme legcons:Item .

F2021L00310:42 a legcons:Item,
        owl:Class,
        dcat:Resource ;
    rdfs:label "Item - I42 4 7  Secure storage area"@en-AU ;
    dct:isPartOf F2021L00310:35 ;
    dct:isReferencedBy F2021L00310: ;
    rdfs:comment "4 7  Secure storage area - Abrievated Graph Key: I42"@en-AU ;
    skos:definition "4 7  Secure storage area"@en-AU ;
    skos:narrower F2021L00310:35 ;
    skos:prefLabel "Item I42"@en-AU ;
    dcat:accessURL <https://www.legislation.gov.au/F2021L00310/2023-08-04/2023-08-04/text/1/epub/OEBPS/document_1/document_1.html#_Toc145601368> ;
    dcat:landingPage "https://www.legislation.gov.au/F2021L00310/2023-08-04/2023-08-04/text/1/epub/OEBPS/document_1/document_1.html#_Toc145601368"^^xsd:anyURI ;
    dcat:theme legcons:Item .

F2021L00310:43 a legcons:Item,
        owl:Class,
        dcat:Resource ;
    rdfs:label "Item - I43 4 8  Amenities for Commonwealth authorised officers"@en-AU ;
    dct:isPartOf F2021L00310:35 ;
    dct:isReferencedBy F2021L00310: ;
    rdfs:comment "4 8  Amenities for Commonwealth authorised officers - Abrievated Graph Key: I43"@en-AU ;
    skos:definition "4 8  Amenities for Commonwealth authorised officers"@en-AU ;
    skos:narrower F2021L00310:35 ;
    skos:prefLabel "Item I43"@en-AU ;
    dcat:accessURL <https://www.legislation.gov.au/F2021L00310/2023-08-04/2023-08-04/text/1/epub/OEBPS/document_1/document_1.html#_Toc145601369> ;
    dcat:landingPage "https://www.legislation.gov.au/F2021L00310/2023-08-04/2023-08-04/text/1/epub/OEBPS/document_1/document_1.html#_Toc145601369"^^xsd:anyURI ;
    dcat:theme legcons:Item .

F2021L00310:45 a legcons:Item,
        owl:Class,
        dcat:Resource ;
    rdfs:label "Item - I45 4 9  Purpose of this Part"@en-AU ;
    dct:isPartOf F2021L00310:44 ;
    dct:isReferencedBy F2021L00310: ;
    rdfs:comment "4 9  Purpose of this Part - Abrievated Graph Key: I45"@en-AU ;
    skos:definition "4 9  Purpose of this Part"@en-AU ;
    skos:narrower F2021L00310:44 ;
    skos:prefLabel "Item I45"@en-AU ;
    dcat:accessURL <https://www.legislation.gov.au/F2021L00310/2023-08-04/2023-08-04/text/1/epub/OEBPS/document_1/document_1.html#_Toc145601371> ;
    dcat:landingPage "https://www.legislation.gov.au/F2021L00310/2023-08-04/2023-08-04/text/1/epub/OEBPS/document_1/document_1.html#_Toc145601371"^^xsd:anyURI ;
    dcat:theme legcons:Item .

F2021L00310:46 a legcons:Item,
        owl:Class,
        dcat:Resource ;
    rdfs:label "Item - I46 4 10  Requirements for registration continue to be met"@en-AU ;
    dct:isPartOf F2021L00310:44 ;
    dct:isReferencedBy F2021L00310: ;
    rdfs:comment "4 10  Requirements for registration continue to be met - Abrievated Graph Key: I46"@en-AU ;
    skos:definition "4 10  Requirements for registration continue to be met"@en-AU ;
    skos:narrower F2021L00310:44 ;
    skos:prefLabel "Item I46"@en-AU ;
    dcat:accessURL <https://www.legislation.gov.au/F2021L00310/2023-08-04/2023-08-04/text/1/epub/OEBPS/document_1/document_1.html#_Toc145601372> ;
    dcat:landingPage "https://www.legislation.gov.au/F2021L00310/2023-08-04/2023-08-04/text/1/epub/OEBPS/document_1/document_1.html#_Toc145601372"^^xsd:anyURI ;
    dcat:theme legcons:Item .

F2021L00310:47 a legcons:Item,
        owl:Class,
        dcat:Resource ;
    rdfs:label "Item - I47 4 11  Certificate of registration must be displayed"@en-AU ;
    dct:isPartOf F2021L00310:44 ;
    dct:isReferencedBy F2021L00310: ;
    rdfs:comment "4 11  Certificate of registration must be displayed - Abrievated Graph Key: I47"@en-AU ;
    skos:definition "4 11  Certificate of registration must be displayed"@en-AU ;
    skos:narrower F2021L00310:44 ;
    skos:prefLabel "Item I47"@en-AU ;
    dcat:accessURL <https://www.legislation.gov.au/F2021L00310/2023-08-04/2023-08-04/text/1/epub/OEBPS/document_1/document_1.html#_Toc145601373> ;
    dcat:landingPage "https://www.legislation.gov.au/F2021L00310/2023-08-04/2023-08-04/text/1/epub/OEBPS/document_1/document_1.html#_Toc145601373"^^xsd:anyURI ;
    dcat:theme legcons:Item .

F2021L00310:48 a legcons:Item,
        owl:Class,
        dcat:Resource ;
    rdfs:label "Item - I48 4 12  Notice of certain matters must be given to persons who manage or control export operations at registered establishment"@en-AU ;
    dct:isPartOf F2021L00310:44 ;
    dct:isReferencedBy F2021L00310: ;
    rdfs:comment "4 12  Notice of certain matters must be given to persons who manage or control export operations at registered establishment - Abrievated Graph Key: I48"@en-AU ;
    skos:definition "4 12  Notice of certain matters must be given to persons who manage or control export operations at registered establishment"@en-AU ;
    skos:narrower F2021L00310:44 ;
    skos:prefLabel "Item I48"@en-AU ;
    dcat:accessURL <https://www.legislation.gov.au/F2021L00310/2023-08-04/2023-08-04/text/1/epub/OEBPS/document_1/document_1.html#_Toc145601374> ;
    dcat:landingPage "https://www.legislation.gov.au/F2021L00310/2023-08-04/2023-08-04/text/1/epub/OEBPS/document_1/document_1.html#_Toc145601374"^^xsd:anyURI ;
    dcat:theme legcons:Item .

F2021L00310:49 a legcons:Item,
        owl:Class,
        dcat:Resource ;
    rdfs:label "Item - I49 4 13  List of persons who manage or control export operations at registered establishment"@en-AU ;
    dct:isPartOf F2021L00310:44 ;
    dct:isReferencedBy F2021L00310: ;
    rdfs:comment "4 13  List of persons who manage or control export operations at registered establishment - Abrievated Graph Key: I49"@en-AU ;
    skos:definition "4 13  List of persons who manage or control export operations at registered establishment"@en-AU ;
    skos:narrower F2021L00310:44 ;
    skos:prefLabel "Item I49"@en-AU ;
    dcat:accessURL <https://www.legislation.gov.au/F2021L00310/2023-08-04/2023-08-04/text/1/epub/OEBPS/document_1/document_1.html#_Toc145601375> ;
    dcat:landingPage "https://www.legislation.gov.au/F2021L00310/2023-08-04/2023-08-04/text/1/epub/OEBPS/document_1/document_1.html#_Toc145601375"^^xsd:anyURI ;
    dcat:theme legcons:Item .

F2021L00310:5 a legcons:Item,
        owl:Class,
        dcat:Resource ;
    rdfs:label "Item - I5 1 4  Simplified outline of this instrument"@en-AU ;
    dct:isPartOf F2021L00310:1 ;
    dct:isReferencedBy F2021L00310: ;
    rdfs:comment "1 4  Simplified outline of this instrument - Abrievated Graph Key: I5"@en-AU ;
    skos:definition "1 4  Simplified outline of this instrument"@en-AU ;
    skos:narrower F2021L00310:1 ;
    skos:prefLabel "Item I5"@en-AU ;
    dcat:accessURL <https://www.legislation.gov.au/F2021L00310/2023-08-04/2023-08-04/text/1/epub/OEBPS/document_1/document_1.html#_Toc145601331> ;
    dcat:landingPage "https://www.legislation.gov.au/F2021L00310/2023-08-04/2023-08-04/text/1/epub/OEBPS/document_1/document_1.html#_Toc145601331"^^xsd:anyURI ;
    dcat:theme legcons:Item .

F2021L00310:50 a legcons:Item,
        owl:Class,
        dcat:Resource ;
    rdfs:label "Item - I50 4 14  Meat inspection services"@en-AU ;
    dct:isPartOf F2021L00310:44 ;
    dct:isReferencedBy F2021L00310: ;
    rdfs:comment "4 14  Meat inspection services - Abrievated Graph Key: I50"@en-AU ;
    skos:definition "4 14  Meat inspection services"@en-AU ;
    skos:narrower F2021L00310:44 ;
    skos:prefLabel "Item I50"@en-AU ;
    dcat:accessURL <https://www.legislation.gov.au/F2021L00310/2023-08-04/2023-08-04/text/1/epub/OEBPS/document_1/document_1.html#_Toc145601376> ;
    dcat:landingPage "https://www.legislation.gov.au/F2021L00310/2023-08-04/2023-08-04/text/1/epub/OEBPS/document_1/document_1.html#_Toc145601376"^^xsd:anyURI ;
    dcat:theme legcons:Item .

F2021L00310:52 a legcons:Item,
        owl:Class,
        dcat:Resource ;
    rdfs:label "Item - I52 4 15  Period within which application to renew registration must be made"@en-AU ;
    dct:isPartOf F2021L00310:51 ;
    dct:isReferencedBy F2021L00310: ;
    rdfs:comment "4 15  Period within which application to renew registration must be made - Abrievated Graph Key: I52"@en-AU ;
    skos:definition "4 15  Period within which application to renew registration must be made"@en-AU ;
    skos:narrower F2021L00310:51 ;
    skos:prefLabel "Item I52"@en-AU ;
    dcat:accessURL <https://www.legislation.gov.au/F2021L00310/2023-08-04/2023-08-04/text/1/epub/OEBPS/document_1/document_1.html#_Toc145601378> ;
    dcat:landingPage "https://www.legislation.gov.au/F2021L00310/2023-08-04/2023-08-04/text/1/epub/OEBPS/document_1/document_1.html#_Toc145601378"^^xsd:anyURI ;
    dcat:theme legcons:Item .

F2021L00310:53 a legcons:Item,
        owl:Class,
        dcat:Resource ;
    rdfs:label "Item - I53 4 16  Requirements for renewal of registration"@en-AU ;
    dct:isPartOf F2021L00310:51 ;
    dct:isReferencedBy F2021L00310: ;
    rdfs:comment "4 16  Requirements for renewal of registration - Abrievated Graph Key: I53"@en-AU ;
    skos:definition "4 16  Requirements for renewal of registration"@en-AU ;
    skos:narrower F2021L00310:51 ;
    skos:prefLabel "Item I53"@en-AU ;
    dcat:accessURL <https://www.legislation.gov.au/F2021L00310/2023-08-04/2023-08-04/text/1/epub/OEBPS/document_1/document_1.html#_Toc145601379> ;
    dcat:landingPage "https://www.legislation.gov.au/F2021L00310/2023-08-04/2023-08-04/text/1/epub/OEBPS/document_1/document_1.html#_Toc145601379"^^xsd:anyURI ;
    dcat:theme legcons:Item .

F2021L00310:55 a legcons:Item,
        owl:Class,
        dcat:Resource ;
    rdfs:label "Item - I55 4 17  Alterations for which approval is not required"@en-AU ;
    dct:isPartOf F2021L00310:54 ;
    dct:isReferencedBy F2021L00310: ;
    rdfs:comment "4 17  Alterations for which approval is not required - Abrievated Graph Key: I55"@en-AU ;
    skos:definition "4 17  Alterations for which approval is not required"@en-AU ;
    skos:narrower F2021L00310:54 ;
    skos:prefLabel "Item I55"@en-AU ;
    dcat:accessURL <https://www.legislation.gov.au/F2021L00310/2023-08-04/2023-08-04/text/1/epub/OEBPS/document_1/document_1.html#_Toc145601381> ;
    dcat:landingPage "https://www.legislation.gov.au/F2021L00310/2023-08-04/2023-08-04/text/1/epub/OEBPS/document_1/document_1.html#_Toc145601381"^^xsd:anyURI ;
    dcat:theme legcons:Item .

F2021L00310:57 a legcons:Item,
        owl:Class,
        dcat:Resource ;
    rdfs:label "Item - I57 4 18  Application of this Part"@en-AU ;
    dct:isPartOf F2021L00310:56 ;
    dct:isReferencedBy F2021L00310: ;
    rdfs:comment "4 18  Application of this Part - Abrievated Graph Key: I57"@en-AU ;
    skos:definition "4 18  Application of this Part"@en-AU ;
    skos:narrower F2021L00310:56 ;
    skos:prefLabel "Item I57"@en-AU ;
    dcat:accessURL <https://www.legislation.gov.au/F2021L00310/2023-08-04/2023-08-04/text/1/epub/OEBPS/document_1/document_1.html#_Toc145601383> ;
    dcat:landingPage "https://www.legislation.gov.au/F2021L00310/2023-08-04/2023-08-04/text/1/epub/OEBPS/document_1/document_1.html#_Toc145601383"^^xsd:anyURI ;
    dcat:theme legcons:Item .

F2021L00310:58 a legcons:Item,
        owl:Class,
        dcat:Resource ;
    rdfs:label "Item - I58 4 19  Initial consideration period"@en-AU ;
    dct:isPartOf F2021L00310:56 ;
    dct:isReferencedBy F2021L00310: ;
    rdfs:comment "4 19  Initial consideration period - Abrievated Graph Key: I58"@en-AU ;
    skos:definition "4 19  Initial consideration period"@en-AU ;
    skos:narrower F2021L00310:56 ;
    skos:prefLabel "Item I58"@en-AU ;
    dcat:accessURL <https://www.legislation.gov.au/F2021L00310/2023-08-04/2023-08-04/text/1/epub/OEBPS/document_1/document_1.html#_Toc145601384> ;
    dcat:landingPage "https://www.legislation.gov.au/F2021L00310/2023-08-04/2023-08-04/text/1/epub/OEBPS/document_1/document_1.html#_Toc145601384"^^xsd:anyURI ;
    dcat:theme legcons:Item .

F2021L00310:59 a legcons:Item,
        owl:Class,
        dcat:Resource ;
    rdfs:label "Item - I59 4 20  Period within which request relating to application must be complied with"@en-AU ;
    dct:isPartOf F2021L00310:56 ;
    dct:isReferencedBy F2021L00310: ;
    rdfs:comment "4 20  Period within which request relating to application must be complied with - Abrievated Graph Key: I59"@en-AU ;
    skos:definition "4 20  Period within which request relating to application must be complied with"@en-AU ;
    skos:narrower F2021L00310:56 ;
    skos:prefLabel "Item I59"@en-AU ;
    dcat:accessURL <https://www.legislation.gov.au/F2021L00310/2023-08-04/2023-08-04/text/1/epub/OEBPS/document_1/document_1.html#_Toc145601385> ;
    dcat:landingPage "https://www.legislation.gov.au/F2021L00310/2023-08-04/2023-08-04/text/1/epub/OEBPS/document_1/document_1.html#_Toc145601385"^^xsd:anyURI ;
    dcat:theme legcons:Item .

F2021L00310:6 a legcons:Part,
        owl:Class,
        dcat:Resource ;
    rdfs:label "Part - P6 Part 2 Interpretation"@en-AU ;
    dct:isPartOf F2021L00310:1 ;
    dct:isReferencedBy F2021L00310: ;
    rdfs:comment "Part 2 Interpretation - Abrievated Graph Key: P6"@en-AU ;
    skos:definition "Part 2 Interpretation"@en-AU ;
    skos:narrower F2021L00310:1 ;
    skos:prefLabel "Part P6"@en-AU ;
    dcat:accessURL <https://www.legislation.gov.au/F2021L00310/2023-08-04/2023-08-04/text/1/epub/OEBPS/document_1/document_1.html#_Toc145601332> ;
    dcat:landingPage "https://www.legislation.gov.au/F2021L00310/2023-08-04/2023-08-04/text/1/epub/OEBPS/document_1/document_1.html#_Toc145601332"^^xsd:anyURI ;
    dcat:theme legcons:Part .

F2021L00310:62 a legcons:Item,
        owl:Class,
        dcat:Resource ;
    rdfs:label "Item - I62 4 21  Application for allocation of meat inspection services to establishment"@en-AU ;
    dct:isPartOf F2021L00310:61 ;
    dct:isReferencedBy F2021L00310: ;
    rdfs:comment "4 21  Application for allocation of meat inspection services to establishment - Abrievated Graph Key: I62"@en-AU ;
    skos:definition "4 21  Application for allocation of meat inspection services to establishment"@en-AU ;
    skos:narrower F2021L00310:61 ;
    skos:prefLabel "Item I62"@en-AU ;
    dcat:accessURL <https://www.legislation.gov.au/F2021L00310/2023-08-04/2023-08-04/text/1/epub/OEBPS/document_1/document_1.html#_Toc145601388> ;
    dcat:landingPage "https://www.legislation.gov.au/F2021L00310/2023-08-04/2023-08-04/text/1/epub/OEBPS/document_1/document_1.html#_Toc145601388"^^xsd:anyURI ;
    dcat:theme legcons:Item .

F2021L00310:63 a legcons:Item,
        owl:Class,
        dcat:Resource ;
    rdfs:label "Item - I63 4 22  Preliminary allocation"@en-AU ;
    dct:isPartOf F2021L00310:61 ;
    dct:isReferencedBy F2021L00310: ;
    rdfs:comment "4 22  Preliminary allocation - Abrievated Graph Key: I63"@en-AU ;
    skos:definition "4 22  Preliminary allocation"@en-AU ;
    skos:narrower F2021L00310:61 ;
    skos:prefLabel "Item I63"@en-AU ;
    dcat:accessURL <https://www.legislation.gov.au/F2021L00310/2023-08-04/2023-08-04/text/1/epub/OEBPS/document_1/document_1.html#_Toc145601389> ;
    dcat:landingPage "https://www.legislation.gov.au/F2021L00310/2023-08-04/2023-08-04/text/1/epub/OEBPS/document_1/document_1.html#_Toc145601389"^^xsd:anyURI ;
    dcat:theme legcons:Item .

F2021L00310:64 a legcons:Item,
        owl:Class,
        dcat:Resource ;
    rdfs:label "Item - I64 4 23  Notice of preliminary allocation"@en-AU ;
    dct:isPartOf F2021L00310:61 ;
    dct:isReferencedBy F2021L00310: ;
    rdfs:comment "4 23  Notice of preliminary allocation - Abrievated Graph Key: I64"@en-AU ;
    skos:definition "4 23  Notice of preliminary allocation"@en-AU ;
    skos:narrower F2021L00310:61 ;
    skos:prefLabel "Item I64"@en-AU ;
    dcat:accessURL <https://www.legislation.gov.au/F2021L00310/2023-08-04/2023-08-04/text/1/epub/OEBPS/document_1/document_1.html#_Toc145601390> ;
    dcat:landingPage "https://www.legislation.gov.au/F2021L00310/2023-08-04/2023-08-04/text/1/epub/OEBPS/document_1/document_1.html#_Toc145601390"^^xsd:anyURI ;
    dcat:theme legcons:Item .

F2021L00310:65 a legcons:Item,
        owl:Class,
        dcat:Resource ;
    rdfs:label "Item - I65 4 24  Procedure following notice of preliminary allocation"@en-AU ;
    dct:isPartOf F2021L00310:61 ;
    dct:isReferencedBy F2021L00310: ;
    rdfs:comment "4 24  Procedure following notice of preliminary allocation - Abrievated Graph Key: I65"@en-AU ;
    skos:definition "4 24  Procedure following notice of preliminary allocation"@en-AU ;
    skos:narrower F2021L00310:61 ;
    skos:prefLabel "Item I65"@en-AU ;
    dcat:accessURL <https://www.legislation.gov.au/F2021L00310/2023-08-04/2023-08-04/text/1/epub/OEBPS/document_1/document_1.html#_Toc145601391> ;
    dcat:landingPage "https://www.legislation.gov.au/F2021L00310/2023-08-04/2023-08-04/text/1/epub/OEBPS/document_1/document_1.html#_Toc145601391"^^xsd:anyURI ;
    dcat:theme legcons:Item .

F2021L00310:66 a legcons:Item,
        owl:Class,
        dcat:Resource ;
    rdfs:label "Item - I66 4 25  Revised allocation"@en-AU ;
    dct:isPartOf F2021L00310:61 ;
    dct:isReferencedBy F2021L00310: ;
    rdfs:comment "4 25  Revised allocation - Abrievated Graph Key: I66"@en-AU ;
    skos:definition "4 25  Revised allocation"@en-AU ;
    skos:narrower F2021L00310:61 ;
    skos:prefLabel "Item I66"@en-AU ;
    dcat:accessURL <https://www.legislation.gov.au/F2021L00310/2023-08-04/2023-08-04/text/1/epub/OEBPS/document_1/document_1.html#_Toc145601392> ;
    dcat:landingPage "https://www.legislation.gov.au/F2021L00310/2023-08-04/2023-08-04/text/1/epub/OEBPS/document_1/document_1.html#_Toc145601392"^^xsd:anyURI ;
    dcat:theme legcons:Item .

F2021L00310:67 a legcons:Item,
        owl:Class,
        dcat:Resource ;
    rdfs:label "Item - I67 4 26  Procedure following notice of revised allocation"@en-AU ;
    dct:isPartOf F2021L00310:61 ;
    dct:isReferencedBy F2021L00310: ;
    rdfs:comment "4 26  Procedure following notice of revised allocation - Abrievated Graph Key: I67"@en-AU ;
    skos:definition "4 26  Procedure following notice of revised allocation"@en-AU ;
    skos:narrower F2021L00310:61 ;
    skos:prefLabel "Item I67"@en-AU ;
    dcat:accessURL <https://www.legislation.gov.au/F2021L00310/2023-08-04/2023-08-04/text/1/epub/OEBPS/document_1/document_1.html#_Toc145601393> ;
    dcat:landingPage "https://www.legislation.gov.au/F2021L00310/2023-08-04/2023-08-04/text/1/epub/OEBPS/document_1/document_1.html#_Toc145601393"^^xsd:anyURI ;
    dcat:theme legcons:Item .

F2021L00310:68 a legcons:Item,
        owl:Class,
        dcat:Resource ;
    rdfs:label "Item - I68 4 27  Review of Secretarys determination"@en-AU ;
    dct:isPartOf F2021L00310:61 ;
    dct:isReferencedBy F2021L00310: ;
    rdfs:comment "4 27  Review of Secretarys determination - Abrievated Graph Key: I68"@en-AU ;
    skos:definition "4 27  Review of Secretarys determination"@en-AU ;
    skos:narrower F2021L00310:61 ;
    skos:prefLabel "Item I68"@en-AU ;
    dcat:accessURL <https://www.legislation.gov.au/F2021L00310/2023-08-04/2023-08-04/text/1/epub/OEBPS/document_1/document_1.html#_Toc145601394> ;
    dcat:landingPage "https://www.legislation.gov.au/F2021L00310/2023-08-04/2023-08-04/text/1/epub/OEBPS/document_1/document_1.html#_Toc145601394"^^xsd:anyURI ;
    dcat:theme legcons:Item .

F2021L00310:69 a legcons:Item,
        owl:Class,
        dcat:Resource ;
    rdfs:label "Item - I69 4 28  Determination of new allocation"@en-AU ;
    dct:isPartOf F2021L00310:61 ;
    dct:isReferencedBy F2021L00310: ;
    rdfs:comment "4 28  Determination of new allocation - Abrievated Graph Key: I69"@en-AU ;
    skos:definition "4 28  Determination of new allocation"@en-AU ;
    skos:narrower F2021L00310:61 ;
    skos:prefLabel "Item I69"@en-AU ;
    dcat:accessURL <https://www.legislation.gov.au/F2021L00310/2023-08-04/2023-08-04/text/1/epub/OEBPS/document_1/document_1.html#_Toc145601395> ;
    dcat:landingPage "https://www.legislation.gov.au/F2021L00310/2023-08-04/2023-08-04/text/1/epub/OEBPS/document_1/document_1.html#_Toc145601395"^^xsd:anyURI ;
    dcat:theme legcons:Item .

F2021L00310:7 a legcons:Division,
        owl:Class,
        dcat:Resource ;
    rdfs:label "Division - D7 Division 1 Definitions"@en-AU ;
    dct:isPartOf F2021L00310:1 ;
    dct:isReferencedBy F2021L00310: ;
    rdfs:comment "Division 1 Definitions - Abrievated Graph Key: D7"@en-AU ;
    skos:definition "Division 1 Definitions"@en-AU ;
    skos:narrower F2021L00310:1 ;
    skos:prefLabel "Division D7"@en-AU ;
    dcat:accessURL <https://www.legislation.gov.au/F2021L00310/2023-08-04/2023-08-04/text/1/epub/OEBPS/document_1/document_1.html#_Toc145601333> ;
    dcat:landingPage "https://www.legislation.gov.au/F2021L00310/2023-08-04/2023-08-04/text/1/epub/OEBPS/document_1/document_1.html#_Toc145601333"^^xsd:anyURI ;
    dcat:theme legcons:Division .

F2021L00310:71 a legcons:Item,
        owl:Class,
        dcat:Resource ;
    rdfs:label "Item - I71 4 29  Application to vary allocation of meat inspection services"@en-AU ;
    dct:isPartOf F2021L00310:70 ;
    dct:isReferencedBy F2021L00310: ;
    rdfs:comment "4 29  Application to vary allocation of meat inspection services - Abrievated Graph Key: I71"@en-AU ;
    skos:definition "4 29  Application to vary allocation of meat inspection services"@en-AU ;
    skos:narrower F2021L00310:70 ;
    skos:prefLabel "Item I71"@en-AU ;
    dcat:accessURL <https://www.legislation.gov.au/F2021L00310/2023-08-04/2023-08-04/text/1/epub/OEBPS/document_1/document_1.html#_Toc145601397> ;
    dcat:landingPage "https://www.legislation.gov.au/F2021L00310/2023-08-04/2023-08-04/text/1/epub/OEBPS/document_1/document_1.html#_Toc145601397"^^xsd:anyURI ;
    dcat:theme legcons:Item .

F2021L00310:72 a legcons:Item,
        owl:Class,
        dcat:Resource ;
    rdfs:label "Item - I72 4 30  Application for additional allocation of meat inspection services"@en-AU ;
    dct:isPartOf F2021L00310:70 ;
    dct:isReferencedBy F2021L00310: ;
    rdfs:comment "4 30  Application for additional allocation of meat inspection services - Abrievated Graph Key: I72"@en-AU ;
    skos:definition "4 30  Application for additional allocation of meat inspection services"@en-AU ;
    skos:narrower F2021L00310:70 ;
    skos:prefLabel "Item I72"@en-AU ;
    dcat:accessURL <https://www.legislation.gov.au/F2021L00310/2023-08-04/2023-08-04/text/1/epub/OEBPS/document_1/document_1.html#_Toc145601398> ;
    dcat:landingPage "https://www.legislation.gov.au/F2021L00310/2023-08-04/2023-08-04/text/1/epub/OEBPS/document_1/document_1.html#_Toc145601398"^^xsd:anyURI ;
    dcat:theme legcons:Item .

F2021L00310:73 a legcons:Item,
        owl:Class,
        dcat:Resource ;
    rdfs:label "Item - I73 4 31  Notification that meat inspection services not required during shutdown period"@en-AU ;
    dct:isPartOf F2021L00310:70 ;
    dct:isReferencedBy F2021L00310: ;
    rdfs:comment "4 31  Notification that meat inspection services not required during shutdown period - Abrievated Graph Key: I73"@en-AU ;
    skos:definition "4 31  Notification that meat inspection services not required during shutdown period"@en-AU ;
    skos:narrower F2021L00310:70 ;
    skos:prefLabel "Item I73"@en-AU ;
    dcat:accessURL <https://www.legislation.gov.au/F2021L00310/2023-08-04/2023-08-04/text/1/epub/OEBPS/document_1/document_1.html#_Toc145601399> ;
    dcat:landingPage "https://www.legislation.gov.au/F2021L00310/2023-08-04/2023-08-04/text/1/epub/OEBPS/document_1/document_1.html#_Toc145601399"^^xsd:anyURI ;
    dcat:theme legcons:Item .

F2021L00310:74 a legcons:Item,
        owl:Class,
        dcat:Resource ;
    rdfs:label "Item - I74 4 32  Variation by Secretary of allocation of meat inspection services"@en-AU ;
    dct:isPartOf F2021L00310:70 ;
    dct:isReferencedBy F2021L00310: ;
    rdfs:comment "4 32  Variation by Secretary of allocation of meat inspection services - Abrievated Graph Key: I74"@en-AU ;
    skos:definition "4 32  Variation by Secretary of allocation of meat inspection services"@en-AU ;
    skos:narrower F2021L00310:70 ;
    skos:prefLabel "Item I74"@en-AU ;
    dcat:accessURL <https://www.legislation.gov.au/F2021L00310/2023-08-04/2023-08-04/text/1/epub/OEBPS/document_1/document_1.html#_Toc145601400> ;
    dcat:landingPage "https://www.legislation.gov.au/F2021L00310/2023-08-04/2023-08-04/text/1/epub/OEBPS/document_1/document_1.html#_Toc145601400"^^xsd:anyURI ;
    dcat:theme legcons:Item .

F2021L00310:75 a legcons:Item,
        owl:Class,
        dcat:Resource ;
    rdfs:label "Item - I75 4 33  Notification of termination of meat inspection services"@en-AU ;
    dct:isPartOf F2021L00310:70 ;
    dct:isReferencedBy F2021L00310: ;
    rdfs:comment "4 33  Notification of termination of meat inspection services - Abrievated Graph Key: I75"@en-AU ;
    skos:definition "4 33  Notification of termination of meat inspection services"@en-AU ;
    skos:narrower F2021L00310:70 ;
    skos:prefLabel "Item I75"@en-AU ;
    dcat:accessURL <https://www.legislation.gov.au/F2021L00310/2023-08-04/2023-08-04/text/1/epub/OEBPS/document_1/document_1.html#_Toc145601401> ;
    dcat:landingPage "https://www.legislation.gov.au/F2021L00310/2023-08-04/2023-08-04/text/1/epub/OEBPS/document_1/document_1.html#_Toc145601401"^^xsd:anyURI ;
    dcat:theme legcons:Item .

F2021L00310:78 a legcons:Item,
        owl:Class,
        dcat:Resource ;
    rdfs:label "Item - I78 5 1  Purpose of this Part"@en-AU ;
    dct:isPartOf F2021L00310:77 ;
    dct:isReferencedBy F2021L00310: ;
    rdfs:comment "5 1  Purpose of this Part - Abrievated Graph Key: I78"@en-AU ;
    skos:definition "5 1  Purpose of this Part"@en-AU ;
    skos:narrower F2021L00310:77 ;
    skos:prefLabel "Item I78"@en-AU ;
    dcat:accessURL <https://www.legislation.gov.au/F2021L00310/2023-08-04/2023-08-04/text/1/epub/OEBPS/document_1/document_1.html#_Toc145601404> ;
    dcat:landingPage "https://www.legislation.gov.au/F2021L00310/2023-08-04/2023-08-04/text/1/epub/OEBPS/document_1/document_1.html#_Toc145601404"^^xsd:anyURI ;
    dcat:theme legcons:Item .

F2021L00310:79 a legcons:Item,
        owl:Class,
        dcat:Resource ;
    rdfs:label "Item - I79 5 2  Other requirementsproposed arrangement for operations to prepare prescribed poultry meat or poultry meat products"@en-AU ;
    dct:isPartOf F2021L00310:77 ;
    dct:isReferencedBy F2021L00310: ;
    rdfs:comment "5 2  Other requirementsproposed arrangement for operations to prepare prescribed poultry meat or poultry meat products - Abrievated Graph Key: I79"@en-AU ;
    skos:definition "5 2  Other requirementsproposed arrangement for operations to prepare prescribed poultry meat or poultry meat products"@en-AU ;
    skos:narrower F2021L00310:77 ;
    skos:prefLabel "Item I79"@en-AU ;
    dcat:accessURL <https://www.legislation.gov.au/F2021L00310/2023-08-04/2023-08-04/text/1/epub/OEBPS/document_1/document_1.html#_Toc145601405> ;
    dcat:landingPage "https://www.legislation.gov.au/F2021L00310/2023-08-04/2023-08-04/text/1/epub/OEBPS/document_1/document_1.html#_Toc145601405"^^xsd:anyURI ;
    dcat:theme legcons:Item .

F2021L00310:8 a legcons:Item,
        owl:Class,
        dcat:Resource ;
    rdfs:label "Item - I8 1 5  Definitions"@en-AU ;
    dct:isPartOf F2021L00310:1 ;
    dct:isReferencedBy F2021L00310: ;
    rdfs:comment "1 5  Definitions - Abrievated Graph Key: I8"@en-AU ;
    skos:definition "1 5  Definitions"@en-AU ;
    skos:narrower F2021L00310:1 ;
    skos:prefLabel "Item I8"@en-AU ;
    dcat:accessURL <https://www.legislation.gov.au/F2021L00310/2023-08-04/2023-08-04/text/1/epub/OEBPS/document_1/document_1.html#_Toc145601334> ;
    dcat:landingPage "https://www.legislation.gov.au/F2021L00310/2023-08-04/2023-08-04/text/1/epub/OEBPS/document_1/document_1.html#_Toc145601334"^^xsd:anyURI ;
    dcat:theme legcons:Item .

F2021L00310:82 a legcons:Item,
        owl:Class,
        dcat:Resource ;
    rdfs:label "Item - I82 5 3  Purpose of this Part"@en-AU ;
    dct:isPartOf F2021L00310:81 ;
    dct:isReferencedBy F2021L00310: ;
    rdfs:comment "5 3  Purpose of this Part - Abrievated Graph Key: I82"@en-AU ;
    skos:definition "5 3  Purpose of this Part"@en-AU ;
    skos:narrower F2021L00310:81 ;
    skos:prefLabel "Item I82"@en-AU ;
    dcat:accessURL <https://www.legislation.gov.au/F2021L00310/2023-08-04/2023-08-04/text/1/epub/OEBPS/document_1/document_1.html#_Toc145601408> ;
    dcat:landingPage "https://www.legislation.gov.au/F2021L00310/2023-08-04/2023-08-04/text/1/epub/OEBPS/document_1/document_1.html#_Toc145601408"^^xsd:anyURI ;
    dcat:theme legcons:Item .

F2021L00310:84 a legcons:Item,
        owl:Class,
        dcat:Resource ;
    rdfs:label "Item - I84 5 4  Importing country requirements must be met"@en-AU ;
    dct:isPartOf F2021L00310:83 ;
    dct:isReferencedBy F2021L00310: ;
    rdfs:comment "5 4  Importing country requirements must be met - Abrievated Graph Key: I84"@en-AU ;
    skos:definition "5 4  Importing country requirements must be met"@en-AU ;
    skos:narrower F2021L00310:83 ;
    skos:prefLabel "Item I84"@en-AU ;
    dcat:accessURL <https://www.legislation.gov.au/F2021L00310/2023-08-04/2023-08-04/text/1/epub/OEBPS/document_1/document_1.html#_Toc145601410> ;
    dcat:landingPage "https://www.legislation.gov.au/F2021L00310/2023-08-04/2023-08-04/text/1/epub/OEBPS/document_1/document_1.html#_Toc145601410"^^xsd:anyURI ;
    dcat:theme legcons:Item .

F2021L00310:85 a legcons:Item,
        owl:Class,
        dcat:Resource ;
    rdfs:label "Item - I85 5 5  Requirements of Australian Poultry Meat Standard must be met"@en-AU ;
    dct:isPartOf F2021L00310:83 ;
    dct:isReferencedBy F2021L00310: ;
    rdfs:comment "5 5  Requirements of Australian Poultry Meat Standard must be met - Abrievated Graph Key: I85"@en-AU ;
    skos:definition "5 5  Requirements of Australian Poultry Meat Standard must be met"@en-AU ;
    skos:narrower F2021L00310:83 ;
    skos:prefLabel "Item I85"@en-AU ;
    dcat:accessURL <https://www.legislation.gov.au/F2021L00310/2023-08-04/2023-08-04/text/1/epub/OEBPS/document_1/document_1.html#_Toc145601411> ;
    dcat:landingPage "https://www.legislation.gov.au/F2021L00310/2023-08-04/2023-08-04/text/1/epub/OEBPS/document_1/document_1.html#_Toc145601411"^^xsd:anyURI ;
    dcat:theme legcons:Item .

F2021L00310:87 a legcons:Item,
        owl:Class,
        dcat:Resource ;
    rdfs:label "Item - I87 5 6  Humane treatment of poultry"@en-AU ;
    dct:isPartOf F2021L00310:86 ;
    dct:isReferencedBy F2021L00310: ;
    rdfs:comment "5 6  Humane treatment of poultry - Abrievated Graph Key: I87"@en-AU ;
    skos:definition "5 6  Humane treatment of poultry"@en-AU ;
    skos:narrower F2021L00310:86 ;
    skos:prefLabel "Item I87"@en-AU ;
    dcat:accessURL <https://www.legislation.gov.au/F2021L00310/2023-08-04/2023-08-04/text/1/epub/OEBPS/document_1/document_1.html#_Toc145601413> ;
    dcat:landingPage "https://www.legislation.gov.au/F2021L00310/2023-08-04/2023-08-04/text/1/epub/OEBPS/document_1/document_1.html#_Toc145601413"^^xsd:anyURI ;
    dcat:theme legcons:Item .

F2021L00310:88 a legcons:Item,
        owl:Class,
        dcat:Resource ;
    rdfs:label "Item - I88 5 7  Poultry fat"@en-AU ;
    dct:isPartOf F2021L00310:86 ;
    dct:isReferencedBy F2021L00310: ;
    rdfs:comment "5 7  Poultry fat - Abrievated Graph Key: I88"@en-AU ;
    skos:definition "5 7  Poultry fat"@en-AU ;
    skos:narrower F2021L00310:86 ;
    skos:prefLabel "Item I88"@en-AU ;
    dcat:accessURL <https://www.legislation.gov.au/F2021L00310/2023-08-04/2023-08-04/text/1/epub/OEBPS/document_1/document_1.html#_Toc145601414> ;
    dcat:landingPage "https://www.legislation.gov.au/F2021L00310/2023-08-04/2023-08-04/text/1/epub/OEBPS/document_1/document_1.html#_Toc145601414"^^xsd:anyURI ;
    dcat:theme legcons:Item .

F2021L00310:89 a legcons:Item,
        owl:Class,
        dcat:Resource ;
    rdfs:label "Item - I89 5 8  Dressing poultry"@en-AU ;
    dct:isPartOf F2021L00310:86 ;
    dct:isReferencedBy F2021L00310: ;
    rdfs:comment "5 8  Dressing poultry - Abrievated Graph Key: I89"@en-AU ;
    skos:definition "5 8  Dressing poultry"@en-AU ;
    skos:narrower F2021L00310:86 ;
    skos:prefLabel "Item I89"@en-AU ;
    dcat:accessURL <https://www.legislation.gov.au/F2021L00310/2023-08-04/2023-08-04/text/1/epub/OEBPS/document_1/document_1.html#_Toc145601415> ;
    dcat:landingPage "https://www.legislation.gov.au/F2021L00310/2023-08-04/2023-08-04/text/1/epub/OEBPS/document_1/document_1.html#_Toc145601415"^^xsd:anyURI ;
    dcat:theme legcons:Item .

F2021L00310:9 a legcons:Item,
        owl:Class,
        dcat:Resource ;
    rdfs:label "Item - I9 1 6  Meaning of loaded for export"@en-AU ;
    dct:isPartOf F2021L00310:1 ;
    dct:isReferencedBy F2021L00310: ;
    rdfs:comment "1 6  Meaning of loaded for export - Abrievated Graph Key: I9"@en-AU ;
    skos:definition "1 6  Meaning of loaded for export"@en-AU ;
    skos:narrower F2021L00310:1 ;
    skos:prefLabel "Item I9"@en-AU ;
    dcat:accessURL <https://www.legislation.gov.au/F2021L00310/2023-08-04/2023-08-04/text/1/epub/OEBPS/document_1/document_1.html#_Toc145601335> ;
    dcat:landingPage "https://www.legislation.gov.au/F2021L00310/2023-08-04/2023-08-04/text/1/epub/OEBPS/document_1/document_1.html#_Toc145601335"^^xsd:anyURI ;
    dcat:theme legcons:Item .

F2021L00310:90 a legcons:Item,
        owl:Class,
        dcat:Resource ;
    rdfs:label "Item - I90 5 9  Areas where post mortem inspections are carried out"@en-AU ;
    dct:isPartOf F2021L00310:86 ;
    dct:isReferencedBy F2021L00310: ;
    rdfs:comment "5 9  Areas where post mortem inspections are carried out - Abrievated Graph Key: I90"@en-AU ;
    skos:definition "5 9  Areas where post mortem inspections are carried out"@en-AU ;
    skos:narrower F2021L00310:86 ;
    skos:prefLabel "Item I90"@en-AU ;
    dcat:accessURL <https://www.legislation.gov.au/F2021L00310/2023-08-04/2023-08-04/text/1/epub/OEBPS/document_1/document_1.html#_Toc145601416> ;
    dcat:landingPage "https://www.legislation.gov.au/F2021L00310/2023-08-04/2023-08-04/text/1/epub/OEBPS/document_1/document_1.html#_Toc145601416"^^xsd:anyURI ;
    dcat:theme legcons:Item .

F2021L00310:91 a legcons:Item,
        owl:Class,
        dcat:Resource ;
    rdfs:label "Item - I91 5 10  Disposition if carcase parts aggregated"@en-AU ;
    dct:isPartOf F2021L00310:86 ;
    dct:isReferencedBy F2021L00310: ;
    rdfs:comment "5 10  Disposition if carcase parts aggregated - Abrievated Graph Key: I91"@en-AU ;
    skos:definition "5 10  Disposition if carcase parts aggregated"@en-AU ;
    skos:narrower F2021L00310:86 ;
    skos:prefLabel "Item I91"@en-AU ;
    dcat:accessURL <https://www.legislation.gov.au/F2021L00310/2023-08-04/2023-08-04/text/1/epub/OEBPS/document_1/document_1.html#_Toc145601417> ;
    dcat:landingPage "https://www.legislation.gov.au/F2021L00310/2023-08-04/2023-08-04/text/1/epub/OEBPS/document_1/document_1.html#_Toc145601417"^^xsd:anyURI ;
    dcat:theme legcons:Item .

F2021L00310:92 a legcons:Item,
        owl:Class,
        dcat:Resource ;
    rdfs:label "Item - I92 5 11  Compliance with decisions and dispositions"@en-AU ;
    dct:isPartOf F2021L00310:86 ;
    dct:isReferencedBy F2021L00310: ;
    rdfs:comment "5 11  Compliance with decisions and dispositions - Abrievated Graph Key: I92"@en-AU ;
    skos:definition "5 11  Compliance with decisions and dispositions"@en-AU ;
    skos:narrower F2021L00310:86 ;
    skos:prefLabel "Item I92"@en-AU ;
    dcat:accessURL <https://www.legislation.gov.au/F2021L00310/2023-08-04/2023-08-04/text/1/epub/OEBPS/document_1/document_1.html#_Toc145601418> ;
    dcat:landingPage "https://www.legislation.gov.au/F2021L00310/2023-08-04/2023-08-04/text/1/epub/OEBPS/document_1/document_1.html#_Toc145601418"^^xsd:anyURI ;
    dcat:theme legcons:Item .

F2021L00310:93 a legcons:Item,
        owl:Class,
        dcat:Resource ;
    rdfs:label "Item - I93 5 12  Loading prescribed poultry meat or poultry meat products for transfer between registered establishments"@en-AU ;
    dct:isPartOf F2021L00310:86 ;
    dct:isReferencedBy F2021L00310: ;
    rdfs:comment "5 12  Loading prescribed poultry meat or poultry meat products for transfer between registered establishments - Abrievated Graph Key: I93"@en-AU ;
    skos:definition "5 12  Loading prescribed poultry meat or poultry meat products for transfer between registered establishments"@en-AU ;
    skos:narrower F2021L00310:86 ;
    skos:prefLabel "Item I93"@en-AU ;
    dcat:accessURL <https://www.legislation.gov.au/F2021L00310/2023-08-04/2023-08-04/text/1/epub/OEBPS/document_1/document_1.html#_Toc145601419> ;
    dcat:landingPage "https://www.legislation.gov.au/F2021L00310/2023-08-04/2023-08-04/text/1/epub/OEBPS/document_1/document_1.html#_Toc145601419"^^xsd:anyURI ;
    dcat:theme legcons:Item .

F2021L00310:94 a legcons:Item,
        owl:Class,
        dcat:Resource ;
    rdfs:label "Item - I94 5 13  Loading of prescribed poultry meat or poultry meat productssupervision"@en-AU ;
    dct:isPartOf F2021L00310:86 ;
    dct:isReferencedBy F2021L00310: ;
    rdfs:comment "5 13  Loading of prescribed poultry meat or poultry meat productssupervision - Abrievated Graph Key: I94"@en-AU ;
    skos:definition "5 13  Loading of prescribed poultry meat or poultry meat productssupervision"@en-AU ;
    skos:narrower F2021L00310:86 ;
    skos:prefLabel "Item I94"@en-AU ;
    dcat:accessURL <https://www.legislation.gov.au/F2021L00310/2023-08-04/2023-08-04/text/1/epub/OEBPS/document_1/document_1.html#_Toc145601420> ;
    dcat:landingPage "https://www.legislation.gov.au/F2021L00310/2023-08-04/2023-08-04/text/1/epub/OEBPS/document_1/document_1.html#_Toc145601420"^^xsd:anyURI ;
    dcat:theme legcons:Item .

F2021L00310:95 a legcons:Item,
        owl:Class,
        dcat:Resource ;
    rdfs:label "Item - I95 5 14  Prohibitions on loading"@en-AU ;
    dct:isPartOf F2021L00310:86 ;
    dct:isReferencedBy F2021L00310: ;
    rdfs:comment "5 14  Prohibitions on loading - Abrievated Graph Key: I95"@en-AU ;
    skos:definition "5 14  Prohibitions on loading"@en-AU ;
    skos:narrower F2021L00310:86 ;
    skos:prefLabel "Item I95"@en-AU ;
    dcat:accessURL <https://www.legislation.gov.au/F2021L00310/2023-08-04/2023-08-04/text/1/epub/OEBPS/document_1/document_1.html#_Toc145601421> ;
    dcat:landingPage "https://www.legislation.gov.au/F2021L00310/2023-08-04/2023-08-04/text/1/epub/OEBPS/document_1/document_1.html#_Toc145601421"^^xsd:anyURI ;
    dcat:theme legcons:Item .

F2021L00310:96 a legcons:Item,
        owl:Class,
        dcat:Resource ;
    rdfs:label "Item - I96 5 15  Container system units and equipment for loading aircraft and vessels"@en-AU ;
    dct:isPartOf F2021L00310:86 ;
    dct:isReferencedBy F2021L00310: ;
    rdfs:comment "5 15  Container system units and equipment for loading aircraft and vessels - Abrievated Graph Key: I96"@en-AU ;
    skos:definition "5 15  Container system units and equipment for loading aircraft and vessels"@en-AU ;
    skos:narrower F2021L00310:86 ;
    skos:prefLabel "Item I96"@en-AU ;
    dcat:accessURL <https://www.legislation.gov.au/F2021L00310/2023-08-04/2023-08-04/text/1/epub/OEBPS/document_1/document_1.html#_Toc145601422> ;
    dcat:landingPage "https://www.legislation.gov.au/F2021L00310/2023-08-04/2023-08-04/text/1/epub/OEBPS/document_1/document_1.html#_Toc145601422"^^xsd:anyURI ;
    dcat:theme legcons:Item .

F2021L00310:97 a legcons:Item,
        owl:Class,
        dcat:Resource ;
    rdfs:label "Item - I97 5 16  When a bolt seal must be applied to container system unit"@en-AU ;
    dct:isPartOf F2021L00310:86 ;
    dct:isReferencedBy F2021L00310: ;
    rdfs:comment "5 16  When a bolt seal must be applied to container system unit - Abrievated Graph Key: I97"@en-AU ;
    skos:definition "5 16  When a bolt seal must be applied to container system unit"@en-AU ;
    skos:narrower F2021L00310:86 ;
    skos:prefLabel "Item I97"@en-AU ;
    dcat:accessURL <https://www.legislation.gov.au/F2021L00310/2023-08-04/2023-08-04/text/1/epub/OEBPS/document_1/document_1.html#_Toc145601423> ;
    dcat:landingPage "https://www.legislation.gov.au/F2021L00310/2023-08-04/2023-08-04/text/1/epub/OEBPS/document_1/document_1.html#_Toc145601423"^^xsd:anyURI ;
    dcat:theme legcons:Item .

F2021L00310:98 a legcons:Item,
        owl:Class,
        dcat:Resource ;
    rdfs:label "Item - I98 5 17  Poultry meat transport vehicles measuring devices and other equipment"@en-AU ;
    dct:isPartOf F2021L00310:86 ;
    dct:isReferencedBy F2021L00310: ;
    rdfs:comment "5 17  Poultry meat transport vehicles measuring devices and other equipment - Abrievated Graph Key: I98"@en-AU ;
    skos:definition "5 17  Poultry meat transport vehicles measuring devices and other equipment"@en-AU ;
    skos:narrower F2021L00310:86 ;
    skos:prefLabel "Item I98"@en-AU ;
    dcat:accessURL <https://www.legislation.gov.au/F2021L00310/2023-08-04/2023-08-04/text/1/epub/OEBPS/document_1/document_1.html#_Toc145601424> ;
    dcat:landingPage "https://www.legislation.gov.au/F2021L00310/2023-08-04/2023-08-04/text/1/epub/OEBPS/document_1/document_1.html#_Toc145601424"^^xsd:anyURI ;
    dcat:theme legcons:Item .

F2021L00310:118 a legcons:Division,
        owl:Class,
        dcat:Resource ;
    rdfs:label "Division - D118 Division 8 Meat inspection services"@en-AU ;
    dct:hasPart F2021L00310:119 ;
    dct:isPartOf F2021L00310:80 ;
    dct:isReferencedBy F2021L00310: ;
    rdfs:comment "Division 8 Meat inspection services - Abrievated Graph Key: D118"@en-AU ;
    skos:broader F2021L00310:119 ;
    skos:definition "Division 8 Meat inspection services"@en-AU ;
    skos:narrower F2021L00310:80 ;
    skos:prefLabel "Division D118"@en-AU ;
    dcat:accessURL <https://www.legislation.gov.au/F2021L00310/2023-08-04/2023-08-04/text/1/epub/OEBPS/document_1/document_1.html#_Toc145601444> ;
    dcat:landingPage "https://www.legislation.gov.au/F2021L00310/2023-08-04/2023-08-04/text/1/epub/OEBPS/document_1/document_1.html#_Toc145601444"^^xsd:anyURI ;
    dcat:theme legcons:Division .

F2021L00310:125 a legcons:Part,
        owl:Class,
        dcat:Resource ;
    rdfs:label "Part - P125 Part 3 Renewal of approved arrangement"@en-AU ;
    dct:hasPart F2021L00310:126 ;
    dct:isPartOf F2021L00310:76 ;
    dct:isReferencedBy F2021L00310: ;
    rdfs:comment "Part 3 Renewal of approved arrangement - Abrievated Graph Key: P125"@en-AU ;
    skos:broader F2021L00310:126 ;
    skos:definition "Part 3 Renewal of approved arrangement"@en-AU ;
    skos:narrower F2021L00310:76 ;
    skos:prefLabel "Part P125"@en-AU ;
    dcat:accessURL <https://www.legislation.gov.au/F2021L00310/2023-08-04/2023-08-04/text/1/epub/OEBPS/document_1/document_1.html#_Toc145601451> ;
    dcat:landingPage "https://www.legislation.gov.au/F2021L00310/2023-08-04/2023-08-04/text/1/epub/OEBPS/document_1/document_1.html#_Toc145601451"^^xsd:anyURI ;
    dcat:theme legcons:Part .

F2021L00310:131 a legcons:Division,
        owl:Class,
        dcat:Resource ;
    rdfs:label "Division - D131 Division 2 Variations required by Secretary"@en-AU ;
    dct:hasPart F2021L00310:132 ;
    dct:isPartOf F2021L00310:127 ;
    dct:isReferencedBy F2021L00310: ;
    rdfs:comment "Division 2 Variations required by Secretary - Abrievated Graph Key: D131"@en-AU ;
    skos:broader F2021L00310:132 ;
    skos:definition "Division 2 Variations required by Secretary"@en-AU ;
    skos:narrower F2021L00310:127 ;
    skos:prefLabel "Division D131"@en-AU ;
    dcat:accessURL <https://www.legislation.gov.au/F2021L00310/2023-08-04/2023-08-04/text/1/epub/OEBPS/document_1/document_1.html#_Toc145601457> ;
    dcat:landingPage "https://www.legislation.gov.au/F2021L00310/2023-08-04/2023-08-04/text/1/epub/OEBPS/document_1/document_1.html#_Toc145601457"^^xsd:anyURI ;
    dcat:theme legcons:Division .

F2021L00310:138 a legcons:Part,
        owl:Class,
        dcat:Resource ;
    rdfs:label "Part - P138 Part 1 Issue of export permit"@en-AU ;
    dct:hasPart F2021L00310:139 ;
    dct:isPartOf F2021L00310:137 ;
    dct:isReferencedBy F2021L00310: ;
    rdfs:comment "Part 1 Issue of export permit - Abrievated Graph Key: P138"@en-AU ;
    skos:broader F2021L00310:139 ;
    skos:definition "Part 1 Issue of export permit"@en-AU ;
    skos:narrower F2021L00310:137 ;
    skos:prefLabel "Part P138"@en-AU ;
    dcat:accessURL <https://www.legislation.gov.au/F2021L00310/2023-08-04/2023-08-04/text/1/epub/OEBPS/document_1/document_1.html#_Toc145601464> ;
    dcat:landingPage "https://www.legislation.gov.au/F2021L00310/2023-08-04/2023-08-04/text/1/epub/OEBPS/document_1/document_1.html#_Toc145601464"^^xsd:anyURI ;
    dcat:theme legcons:Part .

F2021L00310:197 a legcons:Division,
        owl:Class,
        dcat:Resource ;
    rdfs:label "Division - D197 Division 1 General"@en-AU ;
    dct:hasPart F2021L00310:198 ;
    dct:isPartOf F2021L00310:196 ;
    dct:isReferencedBy F2021L00310: ;
    rdfs:comment "Division 1 General - Abrievated Graph Key: D197"@en-AU ;
    skos:broader F2021L00310:198 ;
    skos:definition "Division 1 General"@en-AU ;
    skos:narrower F2021L00310:196 ;
    skos:prefLabel "Division D197"@en-AU ;
    dcat:accessURL <https://www.legislation.gov.au/F2021L00310/2023-08-04/2023-08-04/text/1/epub/OEBPS/document_1/document_1.html#_Toc145601523> ;
    dcat:landingPage "https://www.legislation.gov.au/F2021L00310/2023-08-04/2023-08-04/text/1/epub/OEBPS/document_1/document_1.html#_Toc145601523"^^xsd:anyURI ;
    dcat:theme legcons:Division .

F2021L00310:216 a legcons:Part,
        owl:Class,
        dcat:Resource ;
    rdfs:label "Part - P216 Part 2 Assessments"@en-AU ;
    dct:hasPart F2021L00310:217 ;
    dct:isPartOf F2021L00310:195 ;
    dct:isReferencedBy F2021L00310: ;
    rdfs:comment "Part 2 Assessments - Abrievated Graph Key: P216"@en-AU ;
    skos:broader F2021L00310:217 ;
    skos:definition "Part 2 Assessments"@en-AU ;
    skos:narrower F2021L00310:195 ;
    skos:prefLabel "Part P216"@en-AU ;
    dcat:accessURL <https://www.legislation.gov.au/F2021L00310/2023-08-04/2023-08-04/text/1/epub/OEBPS/document_1/document_1.html#_Toc145601542> ;
    dcat:landingPage "https://www.legislation.gov.au/F2021L00310/2023-08-04/2023-08-04/text/1/epub/OEBPS/document_1/document_1.html#_Toc145601542"^^xsd:anyURI ;
    dcat:theme legcons:Part .

F2021L00310:218 a legcons:Part,
        owl:Class,
        dcat:Resource ;
    rdfs:label "Part - P218 Part 3 Powers of the Secretary"@en-AU ;
    dct:hasPart F2021L00310:219 ;
    dct:isPartOf F2021L00310:195 ;
    dct:isReferencedBy F2021L00310: ;
    rdfs:comment "Part 3 Powers of the Secretary - Abrievated Graph Key: P218"@en-AU ;
    skos:broader F2021L00310:219 ;
    skos:definition "Part 3 Powers of the Secretary"@en-AU ;
    skos:narrower F2021L00310:195 ;
    skos:prefLabel "Part P218"@en-AU ;
    dcat:accessURL <https://www.legislation.gov.au/F2021L00310/2023-08-04/2023-08-04/text/1/epub/OEBPS/document_1/document_1.html#_Toc145601544> ;
    dcat:landingPage "https://www.legislation.gov.au/F2021L00310/2023-08-04/2023-08-04/text/1/epub/OEBPS/document_1/document_1.html#_Toc145601544"^^xsd:anyURI ;
    dcat:theme legcons:Part .

F2021L00310:221 a legcons:Division,
        owl:Class,
        dcat:Resource ;
    rdfs:label "Division - D221 Division 1 Third party authorised officers"@en-AU ;
    dct:hasPart F2021L00310:222 ;
    dct:isPartOf F2021L00310:220 ;
    dct:isReferencedBy F2021L00310: ;
    rdfs:comment "Division 1 Third party authorised officers - Abrievated Graph Key: D221"@en-AU ;
    skos:broader F2021L00310:222 ;
    skos:definition "Division 1 Third party authorised officers"@en-AU ;
    skos:narrower F2021L00310:220 ;
    skos:prefLabel "Division D221"@en-AU ;
    dcat:accessURL <https://www.legislation.gov.au/F2021L00310/2023-08-04/2023-08-04/text/1/epub/OEBPS/document_1/document_1.html#_Toc145601547> ;
    dcat:landingPage "https://www.legislation.gov.au/F2021L00310/2023-08-04/2023-08-04/text/1/epub/OEBPS/document_1/document_1.html#_Toc145601547"^^xsd:anyURI ;
    dcat:theme legcons:Division .

F2021L00310:236 a legcons:Division,
        owl:Class,
        dcat:Resource ;
    rdfs:label "Division - D236 Division 3 Directions to deal with non compliance with the Act etc"@en-AU ;
    dct:hasPart F2021L00310:237 ;
    dct:isPartOf F2021L00310:220 ;
    dct:isReferencedBy F2021L00310: ;
    rdfs:comment "Division 3 Directions to deal with non compliance with the Act etc - Abrievated Graph Key: D236"@en-AU ;
    skos:broader F2021L00310:237 ;
    skos:definition "Division 3 Directions to deal with non compliance with the Act etc"@en-AU ;
    skos:narrower F2021L00310:220 ;
    skos:prefLabel "Division D236"@en-AU ;
    dcat:accessURL <https://www.legislation.gov.au/F2021L00310/2023-08-04/2023-08-04/text/1/epub/OEBPS/document_1/document_1.html#_Toc145601562> ;
    dcat:landingPage "https://www.legislation.gov.au/F2021L00310/2023-08-04/2023-08-04/text/1/epub/OEBPS/document_1/document_1.html#_Toc145601562"^^xsd:anyURI ;
    dcat:theme legcons:Division .

F2021L00310:238 a legcons:Division,
        owl:Class,
        dcat:Resource ;
    rdfs:label "Division - D238 Division 4 Miscellaneous"@en-AU ;
    dct:hasPart F2021L00310:239 ;
    dct:isPartOf F2021L00310:220 ;
    dct:isReferencedBy F2021L00310: ;
    rdfs:comment "Division 4 Miscellaneous - Abrievated Graph Key: D238"@en-AU ;
    skos:broader F2021L00310:239 ;
    skos:definition "Division 4 Miscellaneous"@en-AU ;
    skos:narrower F2021L00310:220 ;
    skos:prefLabel "Division D238"@en-AU ;
    dcat:accessURL <https://www.legislation.gov.au/F2021L00310/2023-08-04/2023-08-04/text/1/epub/OEBPS/document_1/document_1.html#_Toc145601564> ;
    dcat:landingPage "https://www.legislation.gov.au/F2021L00310/2023-08-04/2023-08-04/text/1/epub/OEBPS/document_1/document_1.html#_Toc145601564"^^xsd:anyURI ;
    dcat:theme legcons:Division .

F2021L00310:240 a legcons:Chapter,
        owl:Class,
        dcat:Resource ;
    rdfs:label "Chapter - C240 Chapter 10 Compliance and enforcement"@en-AU ;
    dct:hasPart F2021L00310:241,
        F2021L00310:242 ;
    dct:isReferencedBy F2021L00310: ;
    rdfs:comment "Chapter 10 Compliance and enforcement - Abrievated Graph Key: C240"@en-AU ;
    skos:broader F2021L00310:241,
        F2021L00310:242 ;
    skos:definition "Chapter 10 Compliance and enforcement"@en-AU ;
    skos:prefLabel "Chapter C240"@en-AU ;
    dcat:accessURL <https://www.legislation.gov.au/F2021L00310/2023-08-04/2023-08-04/text/1/epub/OEBPS/document_1/document_1.html#_Toc145601566> ;
    dcat:landingPage "https://www.legislation.gov.au/F2021L00310/2023-08-04/2023-08-04/text/1/epub/OEBPS/document_1/document_1.html#_Toc145601566"^^xsd:anyURI ;
    dcat:theme legcons:Chapter .

F2021L00310:244 a legcons:Part,
        owl:Class,
        dcat:Resource ;
    rdfs:label "Part - P244 Part 1 Review of decisions"@en-AU ;
    dct:hasPart F2021L00310:245 ;
    dct:isPartOf F2021L00310:243 ;
    dct:isReferencedBy F2021L00310: ;
    rdfs:comment "Part 1 Review of decisions - Abrievated Graph Key: P244"@en-AU ;
    skos:broader F2021L00310:245 ;
    skos:definition "Part 1 Review of decisions"@en-AU ;
    skos:narrower F2021L00310:243 ;
    skos:prefLabel "Part P244"@en-AU ;
    dcat:accessURL <https://www.legislation.gov.au/F2021L00310/2023-08-04/2023-08-04/text/1/epub/OEBPS/document_1/document_1.html#_Toc145601570> ;
    dcat:landingPage "https://www.legislation.gov.au/F2021L00310/2023-08-04/2023-08-04/text/1/epub/OEBPS/document_1/document_1.html#_Toc145601570"^^xsd:anyURI ;
    dcat:theme legcons:Part .

F2021L00310:257 a legcons:Part,
        owl:Class,
        dcat:Resource ;
    rdfs:label "Part - P257 Part 3 Samples"@en-AU ;
    dct:hasPart F2021L00310:258 ;
    dct:isPartOf F2021L00310:243 ;
    dct:isReferencedBy F2021L00310: ;
    rdfs:comment "Part 3 Samples - Abrievated Graph Key: P257"@en-AU ;
    skos:broader F2021L00310:258 ;
    skos:definition "Part 3 Samples"@en-AU ;
    skos:narrower F2021L00310:243 ;
    skos:prefLabel "Part P257"@en-AU ;
    dcat:accessURL <https://www.legislation.gov.au/F2021L00310/2023-08-04/2023-08-04/text/1/epub/OEBPS/document_1/document_1.html#_Toc145601583> ;
    dcat:landingPage "https://www.legislation.gov.au/F2021L00310/2023-08-04/2023-08-04/text/1/epub/OEBPS/document_1/document_1.html#_Toc145601583"^^xsd:anyURI ;
    dcat:theme legcons:Part .

F2021L00310:262 a legcons:Part,
        owl:Class,
        dcat:Resource ;
    rdfs:label "Part - P262 Part 5 Relevant Commonwealth liabilities"@en-AU ;
    dct:hasPart F2021L00310:263 ;
    dct:isPartOf F2021L00310:243 ;
    dct:isReferencedBy F2021L00310: ;
    rdfs:comment "Part 5 Relevant Commonwealth liabilities - Abrievated Graph Key: P262"@en-AU ;
    skos:broader F2021L00310:263 ;
    skos:definition "Part 5 Relevant Commonwealth liabilities"@en-AU ;
    skos:narrower F2021L00310:243 ;
    skos:prefLabel "Part P262"@en-AU ;
    dcat:accessURL <https://www.legislation.gov.au/F2021L00310/2023-08-04/2023-08-04/text/1/epub/OEBPS/document_1/document_1.html#_Toc145601588> ;
    dcat:landingPage "https://www.legislation.gov.au/F2021L00310/2023-08-04/2023-08-04/text/1/epub/OEBPS/document_1/document_1.html#_Toc145601588"^^xsd:anyURI ;
    dcat:theme legcons:Part .

F2021L00310:265 a legcons:Part,
        owl:Class,
        dcat:Resource ;
    rdfs:label "Part - P265 Part 1 Preliminary"@en-AU ;
    dct:hasPart F2021L00310:266 ;
    dct:isPartOf F2021L00310:264 ;
    dct:isReferencedBy F2021L00310: ;
    rdfs:comment "Part 1 Preliminary - Abrievated Graph Key: P265"@en-AU ;
    skos:broader F2021L00310:266 ;
    skos:definition "Part 1 Preliminary"@en-AU ;
    skos:narrower F2021L00310:264 ;
    skos:prefLabel "Part P265"@en-AU ;
    dcat:accessURL <https://www.legislation.gov.au/F2021L00310/2023-08-04/2023-08-04/text/1/epub/OEBPS/document_1/document_1.html#_Toc145601591> ;
    dcat:landingPage "https://www.legislation.gov.au/F2021L00310/2023-08-04/2023-08-04/text/1/epub/OEBPS/document_1/document_1.html#_Toc145601591"^^xsd:anyURI ;
    dcat:theme legcons:Part .

F2021L00310:285 a legcons:Part,
        owl:Class,
        dcat:Resource ;
    rdfs:label "Part - P285 Part 3 Approved arrangements"@en-AU ;
    dct:hasPart F2021L00310:286 ;
    dct:isPartOf F2021L00310:264 ;
    dct:isReferencedBy F2021L00310: ;
    rdfs:comment "Part 3 Approved arrangements - Abrievated Graph Key: P285"@en-AU ;
    skos:broader F2021L00310:286 ;
    skos:definition "Part 3 Approved arrangements"@en-AU ;
    skos:narrower F2021L00310:264 ;
    skos:prefLabel "Part P285"@en-AU ;
    dcat:accessURL <https://www.legislation.gov.au/F2021L00310/2023-08-04/2023-08-04/text/1/epub/OEBPS/document_1/document_1.html#_Toc145601611> ;
    dcat:landingPage "https://www.legislation.gov.au/F2021L00310/2023-08-04/2023-08-04/text/1/epub/OEBPS/document_1/document_1.html#_Toc145601611"^^xsd:anyURI ;
    dcat:theme legcons:Part .

F2021L00310:288 a legcons:Division,
        owl:Class,
        dcat:Resource ;
    rdfs:label "Division - D288 Division 1 Trade descriptions"@en-AU ;
    dct:hasPart F2021L00310:289 ;
    dct:isPartOf F2021L00310:287 ;
    dct:isReferencedBy F2021L00310: ;
    rdfs:comment "Division 1 Trade descriptions - Abrievated Graph Key: D288"@en-AU ;
    skos:broader F2021L00310:289 ;
    skos:definition "Division 1 Trade descriptions"@en-AU ;
    skos:narrower F2021L00310:287 ;
    skos:prefLabel "Division D288"@en-AU ;
    dcat:accessURL <https://www.legislation.gov.au/F2021L00310/2023-08-04/2023-08-04/text/1/epub/OEBPS/document_1/document_1.html#_Toc145601614> ;
    dcat:landingPage "https://www.legislation.gov.au/F2021L00310/2023-08-04/2023-08-04/text/1/epub/OEBPS/document_1/document_1.html#_Toc145601614"^^xsd:anyURI ;
    dcat:theme legcons:Division .

F2021L00310:54 a legcons:Part,
        owl:Class,
        dcat:Resource ;
    rdfs:label "Part - P54 Part 4 Variation of registration"@en-AU ;
    dct:hasPart F2021L00310:55 ;
    dct:isPartOf F2021L00310:34 ;
    dct:isReferencedBy F2021L00310: ;
    rdfs:comment "Part 4 Variation of registration - Abrievated Graph Key: P54"@en-AU ;
    skos:broader F2021L00310:55 ;
    skos:definition "Part 4 Variation of registration"@en-AU ;
    skos:narrower F2021L00310:34 ;
    skos:prefLabel "Part P54"@en-AU ;
    dcat:accessURL <https://www.legislation.gov.au/F2021L00310/2023-08-04/2023-08-04/text/1/epub/OEBPS/document_1/document_1.html#_Toc145601380> ;
    dcat:landingPage "https://www.legislation.gov.au/F2021L00310/2023-08-04/2023-08-04/text/1/epub/OEBPS/document_1/document_1.html#_Toc145601380"^^xsd:anyURI ;
    dcat:theme legcons:Part .

F2021L00310:81 a legcons:Division,
        owl:Class,
        dcat:Resource ;
    rdfs:label "Division - D81 Division 1 Purpose of this Part"@en-AU ;
    dct:hasPart F2021L00310:82 ;
    dct:isPartOf F2021L00310:80 ;
    dct:isReferencedBy F2021L00310: ;
    rdfs:comment "Division 1 Purpose of this Part - Abrievated Graph Key: D81"@en-AU ;
    skos:broader F2021L00310:82 ;
    skos:definition "Division 1 Purpose of this Part"@en-AU ;
    skos:narrower F2021L00310:80 ;
    skos:prefLabel "Division D81"@en-AU ;
    dcat:accessURL <https://www.legislation.gov.au/F2021L00310/2023-08-04/2023-08-04/text/1/epub/OEBPS/document_1/document_1.html#_Toc145601407> ;
    dcat:landingPage "https://www.legislation.gov.au/F2021L00310/2023-08-04/2023-08-04/text/1/epub/OEBPS/document_1/document_1.html#_Toc145601407"^^xsd:anyURI ;
    dcat:theme legcons:Division .

F2021L00310:115 a legcons:Division,
        owl:Class,
        dcat:Resource ;
    rdfs:label "Division - D115 Division 7 Transfers"@en-AU ;
    dct:hasPart F2021L00310:116,
        F2021L00310:117 ;
    dct:isPartOf F2021L00310:80 ;
    dct:isReferencedBy F2021L00310: ;
    rdfs:comment "Division 7 Transfers - Abrievated Graph Key: D115"@en-AU ;
    skos:broader F2021L00310:116,
        F2021L00310:117 ;
    skos:definition "Division 7 Transfers"@en-AU ;
    skos:narrower F2021L00310:80 ;
    skos:prefLabel "Division D115"@en-AU ;
    dcat:accessURL <https://www.legislation.gov.au/F2021L00310/2023-08-04/2023-08-04/text/1/epub/OEBPS/document_1/document_1.html#_Toc145601441> ;
    dcat:landingPage "https://www.legislation.gov.au/F2021L00310/2023-08-04/2023-08-04/text/1/epub/OEBPS/document_1/document_1.html#_Toc145601441"^^xsd:anyURI ;
    dcat:theme legcons:Division .

F2021L00310:127 a legcons:Part,
        owl:Class,
        dcat:Resource ;
    rdfs:label "Part - P127 Part 4 Variation of approved arrangement"@en-AU ;
    dct:hasPart F2021L00310:128,
        F2021L00310:131 ;
    dct:isPartOf F2021L00310:76 ;
    dct:isReferencedBy F2021L00310: ;
    rdfs:comment "Part 4 Variation of approved arrangement - Abrievated Graph Key: P127"@en-AU ;
    skos:broader F2021L00310:128,
        F2021L00310:131 ;
    skos:definition "Part 4 Variation of approved arrangement"@en-AU ;
    skos:narrower F2021L00310:76 ;
    skos:prefLabel "Part P127"@en-AU ;
    dcat:accessURL <https://www.legislation.gov.au/F2021L00310/2023-08-04/2023-08-04/text/1/epub/OEBPS/document_1/document_1.html#_Toc145601453> ;
    dcat:landingPage "https://www.legislation.gov.au/F2021L00310/2023-08-04/2023-08-04/text/1/epub/OEBPS/document_1/document_1.html#_Toc145601453"^^xsd:anyURI ;
    dcat:theme legcons:Part .

F2021L00310:128 a legcons:Division,
        owl:Class,
        dcat:Resource ;
    rdfs:label "Division - D128 Division 1 Variations by holder"@en-AU ;
    dct:hasPart F2021L00310:129,
        F2021L00310:130 ;
    dct:isPartOf F2021L00310:127 ;
    dct:isReferencedBy F2021L00310: ;
    rdfs:comment "Division 1 Variations by holder - Abrievated Graph Key: D128"@en-AU ;
    skos:broader F2021L00310:129,
        F2021L00310:130 ;
    skos:definition "Division 1 Variations by holder"@en-AU ;
    skos:narrower F2021L00310:127 ;
    skos:prefLabel "Division D128"@en-AU ;
    dcat:accessURL <https://www.legislation.gov.au/F2021L00310/2023-08-04/2023-08-04/text/1/epub/OEBPS/document_1/document_1.html#_Toc145601454> ;
    dcat:landingPage "https://www.legislation.gov.au/F2021L00310/2023-08-04/2023-08-04/text/1/epub/OEBPS/document_1/document_1.html#_Toc145601454"^^xsd:anyURI ;
    dcat:theme legcons:Division .

F2021L00310:13 a legcons:Chapter,
        owl:Class,
        dcat:Resource ;
    rdfs:label "Chapter - C13 Chapter 2 Exporting goods"@en-AU ;
    dct:hasPart F2021L00310:14,
        F2021L00310:21,
        F2021L00310:28 ;
    dct:isReferencedBy F2021L00310: ;
    rdfs:comment "Chapter 2 Exporting goods - Abrievated Graph Key: C13"@en-AU ;
    skos:broader F2021L00310:14,
        F2021L00310:21,
        F2021L00310:28 ;
    skos:definition "Chapter 2 Exporting goods"@en-AU ;
    skos:prefLabel "Chapter C13"@en-AU ;
    dcat:accessURL <https://www.legislation.gov.au/F2021L00310/2023-08-04/2023-08-04/text/1/epub/OEBPS/document_1/document_1.html#_Toc145601339> ;
    dcat:landingPage "https://www.legislation.gov.au/F2021L00310/2023-08-04/2023-08-04/text/1/epub/OEBPS/document_1/document_1.html#_Toc145601339"^^xsd:anyURI ;
    dcat:theme legcons:Chapter .

F2021L00310:137 a legcons:Chapter,
        owl:Class,
        dcat:Resource ;
    rdfs:label "Chapter - C137 Chapter 7 Export permits"@en-AU ;
    dct:hasPart F2021L00310:138,
        F2021L00310:140,
        F2021L00310:144 ;
    dct:isReferencedBy F2021L00310: ;
    rdfs:comment "Chapter 7 Export permits - Abrievated Graph Key: C137"@en-AU ;
    skos:broader F2021L00310:138,
        F2021L00310:140,
        F2021L00310:144 ;
    skos:definition "Chapter 7 Export permits"@en-AU ;
    skos:prefLabel "Chapter C137"@en-AU ;
    dcat:accessURL <https://www.legislation.gov.au/F2021L00310/2023-08-04/2023-08-04/text/1/epub/OEBPS/document_1/document_1.html#_Toc145601463> ;
    dcat:landingPage "https://www.legislation.gov.au/F2021L00310/2023-08-04/2023-08-04/text/1/epub/OEBPS/document_1/document_1.html#_Toc145601463"^^xsd:anyURI ;
    dcat:theme legcons:Chapter .

F2021L00310:14 a legcons:Part,
        owl:Class,
        dcat:Resource ;
    rdfs:label "Part - P14 Part 1 Goods"@en-AU ;
    dct:hasPart F2021L00310:15,
        F2021L00310:18 ;
    dct:isPartOf F2021L00310:13 ;
    dct:isReferencedBy F2021L00310: ;
    rdfs:comment "Part 1 Goods - Abrievated Graph Key: P14"@en-AU ;
    skos:broader F2021L00310:15,
        F2021L00310:18 ;
    skos:definition "Part 1 Goods"@en-AU ;
    skos:narrower F2021L00310:13 ;
    skos:prefLabel "Part P14"@en-AU ;
    dcat:accessURL <https://www.legislation.gov.au/F2021L00310/2023-08-04/2023-08-04/text/1/epub/OEBPS/document_1/document_1.html#_Toc145601340> ;
    dcat:landingPage "https://www.legislation.gov.au/F2021L00310/2023-08-04/2023-08-04/text/1/epub/OEBPS/document_1/document_1.html#_Toc145601340"^^xsd:anyURI ;
    dcat:theme legcons:Part .

F2021L00310:149 a legcons:Chapter,
        owl:Class,
        dcat:Resource ;
    rdfs:label "Chapter - C149 Chapter 8 Other matters relating to export"@en-AU ;
    dct:hasPart F2021L00310:150,
        F2021L00310:155,
        F2021L00310:159 ;
    dct:isReferencedBy F2021L00310: ;
    rdfs:comment "Chapter 8 Other matters relating to export - Abrievated Graph Key: C149"@en-AU ;
    skos:broader F2021L00310:150,
        F2021L00310:155,
        F2021L00310:159 ;
    skos:definition "Chapter 8 Other matters relating to export"@en-AU ;
    skos:prefLabel "Chapter C149"@en-AU ;
    dcat:accessURL <https://www.legislation.gov.au/F2021L00310/2023-08-04/2023-08-04/text/1/epub/OEBPS/document_1/document_1.html#_Toc145601475> ;
    dcat:landingPage "https://www.legislation.gov.au/F2021L00310/2023-08-04/2023-08-04/text/1/epub/OEBPS/document_1/document_1.html#_Toc145601475"^^xsd:anyURI ;
    dcat:theme legcons:Chapter .

F2021L00310:15 a legcons:Division,
        owl:Class,
        dcat:Resource ;
    rdfs:label "Division - D15 Division 1 Prescribed goods"@en-AU ;
    dct:hasPart F2021L00310:16,
        F2021L00310:17 ;
    dct:isPartOf F2021L00310:14 ;
    dct:isReferencedBy F2021L00310: ;
    rdfs:comment "Division 1 Prescribed goods - Abrievated Graph Key: D15"@en-AU ;
    skos:broader F2021L00310:16,
        F2021L00310:17 ;
    skos:definition "Division 1 Prescribed goods"@en-AU ;
    skos:narrower F2021L00310:14 ;
    skos:prefLabel "Division D15"@en-AU ;
    dcat:accessURL <https://www.legislation.gov.au/F2021L00310/2023-08-04/2023-08-04/text/1/epub/OEBPS/document_1/document_1.html#_Toc145601341> ;
    dcat:landingPage "https://www.legislation.gov.au/F2021L00310/2023-08-04/2023-08-04/text/1/epub/OEBPS/document_1/document_1.html#_Toc145601341"^^xsd:anyURI ;
    dcat:theme legcons:Division .

F2021L00310:18 a legcons:Division,
        owl:Class,
        dcat:Resource ;
    rdfs:label "Division - D18 Division 2 Prohibited export and prescribed export conditions"@en-AU ;
    dct:hasPart F2021L00310:19,
        F2021L00310:20 ;
    dct:isPartOf F2021L00310:14 ;
    dct:isReferencedBy F2021L00310: ;
    rdfs:comment "Division 2 Prohibited export and prescribed export conditions - Abrievated Graph Key: D18"@en-AU ;
    skos:broader F2021L00310:19,
        F2021L00310:20 ;
    skos:definition "Division 2 Prohibited export and prescribed export conditions"@en-AU ;
    skos:narrower F2021L00310:14 ;
    skos:prefLabel "Division D18"@en-AU ;
    dcat:accessURL <https://www.legislation.gov.au/F2021L00310/2023-08-04/2023-08-04/text/1/epub/OEBPS/document_1/document_1.html#_Toc145601344> ;
    dcat:landingPage "https://www.legislation.gov.au/F2021L00310/2023-08-04/2023-08-04/text/1/epub/OEBPS/document_1/document_1.html#_Toc145601344"^^xsd:anyURI ;
    dcat:theme legcons:Division .

F2021L00310:259 a legcons:Part,
        owl:Class,
        dcat:Resource ;
    rdfs:label "Part - P259 Part 4 Damaged or destroyed poultry meat or poultry meat products"@en-AU ;
    dct:hasPart F2021L00310:260,
        F2021L00310:261 ;
    dct:isPartOf F2021L00310:243 ;
    dct:isReferencedBy F2021L00310: ;
    rdfs:comment "Part 4 Damaged or destroyed poultry meat or poultry meat products - Abrievated Graph Key: P259"@en-AU ;
    skos:broader F2021L00310:260,
        F2021L00310:261 ;
    skos:definition "Part 4 Damaged or destroyed poultry meat or poultry meat products"@en-AU ;
    skos:narrower F2021L00310:243 ;
    skos:prefLabel "Part P259"@en-AU ;
    dcat:accessURL <https://www.legislation.gov.au/F2021L00310/2023-08-04/2023-08-04/text/1/epub/OEBPS/document_1/document_1.html#_Toc145601585> ;
    dcat:landingPage "https://www.legislation.gov.au/F2021L00310/2023-08-04/2023-08-04/text/1/epub/OEBPS/document_1/document_1.html#_Toc145601585"^^xsd:anyURI ;
    dcat:theme legcons:Part .

F2021L00310:290 a legcons:Division,
        owl:Class,
        dcat:Resource ;
    rdfs:label "Division - D290 Division 2 Official marks"@en-AU ;
    dct:hasPart F2021L00310:291,
        F2021L00310:292 ;
    dct:isPartOf F2021L00310:287 ;
    dct:isReferencedBy F2021L00310: ;
    rdfs:comment "Division 2 Official marks - Abrievated Graph Key: D290"@en-AU ;
    skos:broader F2021L00310:291,
        F2021L00310:292 ;
    skos:definition "Division 2 Official marks"@en-AU ;
    skos:narrower F2021L00310:287 ;
    skos:prefLabel "Division D290"@en-AU ;
    dcat:accessURL <https://www.legislation.gov.au/F2021L00310/2023-08-04/2023-08-04/text/1/epub/OEBPS/document_1/document_1.html#_Toc145601616> ;
    dcat:landingPage "https://www.legislation.gov.au/F2021L00310/2023-08-04/2023-08-04/text/1/epub/OEBPS/document_1/document_1.html#_Toc145601616"^^xsd:anyURI ;
    dcat:theme legcons:Division .

F2021L00310:293 a legcons:Division,
        owl:Class,
        dcat:Resource ;
    rdfs:label "Division - D293 Division 3 Official marking devices"@en-AU ;
    dct:hasPart F2021L00310:294,
        F2021L00310:295 ;
    dct:isPartOf F2021L00310:287 ;
    dct:isReferencedBy F2021L00310: ;
    rdfs:comment "Division 3 Official marking devices - Abrievated Graph Key: D293"@en-AU ;
    skos:broader F2021L00310:294,
        F2021L00310:295 ;
    skos:definition "Division 3 Official marking devices"@en-AU ;
    skos:narrower F2021L00310:287 ;
    skos:prefLabel "Division D293"@en-AU ;
    dcat:accessURL <https://www.legislation.gov.au/F2021L00310/2023-08-04/2023-08-04/text/1/epub/OEBPS/document_1/document_1.html#_Toc145601619> ;
    dcat:landingPage "https://www.legislation.gov.au/F2021L00310/2023-08-04/2023-08-04/text/1/epub/OEBPS/document_1/document_1.html#_Toc145601619"^^xsd:anyURI ;
    dcat:theme legcons:Division .

F2021L00310:296 a legcons:Part,
        owl:Class,
        dcat:Resource ;
    rdfs:label "Part - P296 Part 5 Powers and officials"@en-AU ;
    dct:hasPart F2021L00310:297,
        F2021L00310:301 ;
    dct:isPartOf F2021L00310:264 ;
    dct:isReferencedBy F2021L00310: ;
    rdfs:comment "Part 5 Powers and officials - Abrievated Graph Key: P296"@en-AU ;
    skos:broader F2021L00310:297,
        F2021L00310:301 ;
    skos:definition "Part 5 Powers and officials"@en-AU ;
    skos:narrower F2021L00310:264 ;
    skos:prefLabel "Part P296"@en-AU ;
    dcat:accessURL <https://www.legislation.gov.au/F2021L00310/2023-08-04/2023-08-04/text/1/epub/OEBPS/document_1/document_1.html#_Toc145601622> ;
    dcat:landingPage "https://www.legislation.gov.au/F2021L00310/2023-08-04/2023-08-04/text/1/epub/OEBPS/document_1/document_1.html#_Toc145601622"^^xsd:anyURI ;
    dcat:theme legcons:Part .

F2021L00310:301 a legcons:Division,
        owl:Class,
        dcat:Resource ;
    rdfs:label "Division - D301 Division 2 Decisions and dispositions"@en-AU ;
    dct:hasPart F2021L00310:302,
        F2021L00310:303 ;
    dct:isPartOf F2021L00310:296 ;
    dct:isReferencedBy F2021L00310: ;
    rdfs:comment "Division 2 Decisions and dispositions - Abrievated Graph Key: D301"@en-AU ;
    skos:broader F2021L00310:302,
        F2021L00310:303 ;
    skos:definition "Division 2 Decisions and dispositions"@en-AU ;
    skos:narrower F2021L00310:296 ;
    skos:prefLabel "Division D301"@en-AU ;
    dcat:accessURL <https://www.legislation.gov.au/F2021L00310/2023-08-04/2023-08-04/text/1/epub/OEBPS/document_1/document_1.html#_Toc145601627> ;
    dcat:landingPage "https://www.legislation.gov.au/F2021L00310/2023-08-04/2023-08-04/text/1/epub/OEBPS/document_1/document_1.html#_Toc145601627"^^xsd:anyURI ;
    dcat:theme legcons:Division .

F2021L00310:51 a legcons:Part,
        owl:Class,
        dcat:Resource ;
    rdfs:label "Part - P51 Part 3 Renewal of registration"@en-AU ;
    dct:hasPart F2021L00310:52,
        F2021L00310:53 ;
    dct:isPartOf F2021L00310:34 ;
    dct:isReferencedBy F2021L00310: ;
    rdfs:comment "Part 3 Renewal of registration - Abrievated Graph Key: P51"@en-AU ;
    skos:broader F2021L00310:52,
        F2021L00310:53 ;
    skos:definition "Part 3 Renewal of registration"@en-AU ;
    skos:narrower F2021L00310:34 ;
    skos:prefLabel "Part P51"@en-AU ;
    dcat:accessURL <https://www.legislation.gov.au/F2021L00310/2023-08-04/2023-08-04/text/1/epub/OEBPS/document_1/document_1.html#_Toc145601377> ;
    dcat:landingPage "https://www.legislation.gov.au/F2021L00310/2023-08-04/2023-08-04/text/1/epub/OEBPS/document_1/document_1.html#_Toc145601377"^^xsd:anyURI ;
    dcat:theme legcons:Part .

F2021L00310:60 a legcons:Part,
        owl:Class,
        dcat:Resource ;
    rdfs:label "Part - P60 Part 6 Meat inspection services"@en-AU ;
    dct:hasPart F2021L00310:61,
        F2021L00310:70 ;
    dct:isPartOf F2021L00310:34 ;
    dct:isReferencedBy F2021L00310: ;
    rdfs:comment "Part 6 Meat inspection services - Abrievated Graph Key: P60"@en-AU ;
    skos:broader F2021L00310:61,
        F2021L00310:70 ;
    skos:definition "Part 6 Meat inspection services"@en-AU ;
    skos:narrower F2021L00310:34 ;
    skos:prefLabel "Part P60"@en-AU ;
    dcat:accessURL <https://www.legislation.gov.au/F2021L00310/2023-08-04/2023-08-04/text/1/epub/OEBPS/document_1/document_1.html#_Toc145601386> ;
    dcat:landingPage "https://www.legislation.gov.au/F2021L00310/2023-08-04/2023-08-04/text/1/epub/OEBPS/document_1/document_1.html#_Toc145601386"^^xsd:anyURI ;
    dcat:theme legcons:Part .

F2021L00310:77 a legcons:Part,
        owl:Class,
        dcat:Resource ;
    rdfs:label "Part - P77 Part 1 Requirements for approval"@en-AU ;
    dct:hasPart F2021L00310:78,
        F2021L00310:79 ;
    dct:isPartOf F2021L00310:76 ;
    dct:isReferencedBy F2021L00310: ;
    rdfs:comment "Part 1 Requirements for approval - Abrievated Graph Key: P77"@en-AU ;
    skos:broader F2021L00310:78,
        F2021L00310:79 ;
    skos:definition "Part 1 Requirements for approval"@en-AU ;
    skos:narrower F2021L00310:76 ;
    skos:prefLabel "Part P77"@en-AU ;
    dcat:accessURL <https://www.legislation.gov.au/F2021L00310/2023-08-04/2023-08-04/text/1/epub/OEBPS/document_1/document_1.html#_Toc145601403> ;
    dcat:landingPage "https://www.legislation.gov.au/F2021L00310/2023-08-04/2023-08-04/text/1/epub/OEBPS/document_1/document_1.html#_Toc145601403"^^xsd:anyURI ;
    dcat:theme legcons:Part .

F2021L00310:83 a legcons:Division,
        owl:Class,
        dcat:Resource ;
    rdfs:label "Division - D83 Division 2 General"@en-AU ;
    dct:hasPart F2021L00310:84,
        F2021L00310:85 ;
    dct:isPartOf F2021L00310:80 ;
    dct:isReferencedBy F2021L00310: ;
    rdfs:comment "Division 2 General - Abrievated Graph Key: D83"@en-AU ;
    skos:broader F2021L00310:84,
        F2021L00310:85 ;
    skos:definition "Division 2 General"@en-AU ;
    skos:narrower F2021L00310:80 ;
    skos:prefLabel "Division D83"@en-AU ;
    dcat:accessURL <https://www.legislation.gov.au/F2021L00310/2023-08-04/2023-08-04/text/1/epub/OEBPS/document_1/document_1.html#_Toc145601409> ;
    dcat:landingPage "https://www.legislation.gov.au/F2021L00310/2023-08-04/2023-08-04/text/1/epub/OEBPS/document_1/document_1.html#_Toc145601409"^^xsd:anyURI ;
    dcat:theme legcons:Division .

F2021L00310:133 a legcons:Part,
        owl:Class,
        dcat:Resource ;
    rdfs:label "Part - P133 Part 5 Matters relating to applications"@en-AU ;
    dct:hasPart F2021L00310:134,
        F2021L00310:135,
        F2021L00310:136 ;
    dct:isPartOf F2021L00310:76 ;
    dct:isReferencedBy F2021L00310: ;
    rdfs:comment "Part 5 Matters relating to applications - Abrievated Graph Key: P133"@en-AU ;
    skos:broader F2021L00310:134,
        F2021L00310:135,
        F2021L00310:136 ;
    skos:definition "Part 5 Matters relating to applications"@en-AU ;
    skos:narrower F2021L00310:76 ;
    skos:prefLabel "Part P133"@en-AU ;
    dcat:accessURL <https://www.legislation.gov.au/F2021L00310/2023-08-04/2023-08-04/text/1/epub/OEBPS/document_1/document_1.html#_Toc145601459> ;
    dcat:landingPage "https://www.legislation.gov.au/F2021L00310/2023-08-04/2023-08-04/text/1/epub/OEBPS/document_1/document_1.html#_Toc145601459"^^xsd:anyURI ;
    dcat:theme legcons:Part .

F2021L00310:140 a legcons:Part,
        owl:Class,
        dcat:Resource ;
    rdfs:label "Part - P140 Part 2 Variation suspension and revocation of export permit"@en-AU ;
    dct:hasPart F2021L00310:141,
        F2021L00310:142,
        F2021L00310:143 ;
    dct:isPartOf F2021L00310:137 ;
    dct:isReferencedBy F2021L00310: ;
    rdfs:comment "Part 2 Variation suspension and revocation of export permit - Abrievated Graph Key: P140"@en-AU ;
    skos:broader F2021L00310:141,
        F2021L00310:142,
        F2021L00310:143 ;
    skos:definition "Part 2 Variation suspension and revocation of export permit"@en-AU ;
    skos:narrower F2021L00310:137 ;
    skos:prefLabel "Part P140"@en-AU ;
    dcat:accessURL <https://www.legislation.gov.au/F2021L00310/2023-08-04/2023-08-04/text/1/epub/OEBPS/document_1/document_1.html#_Toc145601466> ;
    dcat:landingPage "https://www.legislation.gov.au/F2021L00310/2023-08-04/2023-08-04/text/1/epub/OEBPS/document_1/document_1.html#_Toc145601466"^^xsd:anyURI ;
    dcat:theme legcons:Part .

F2021L00310:155 a legcons:Part,
        owl:Class,
        dcat:Resource ;
    rdfs:label "Part - P155 Part 2 Trade descriptions"@en-AU ;
    dct:hasPart F2021L00310:156,
        F2021L00310:157,
        F2021L00310:158 ;
    dct:isPartOf F2021L00310:149 ;
    dct:isReferencedBy F2021L00310: ;
    rdfs:comment "Part 2 Trade descriptions - Abrievated Graph Key: P155"@en-AU ;
    skos:broader F2021L00310:156,
        F2021L00310:157,
        F2021L00310:158 ;
    skos:definition "Part 2 Trade descriptions"@en-AU ;
    skos:narrower F2021L00310:149 ;
    skos:prefLabel "Part P155"@en-AU ;
    dcat:accessURL <https://www.legislation.gov.au/F2021L00310/2023-08-04/2023-08-04/text/1/epub/OEBPS/document_1/document_1.html#_Toc145601481> ;
    dcat:landingPage "https://www.legislation.gov.au/F2021L00310/2023-08-04/2023-08-04/text/1/epub/OEBPS/document_1/document_1.html#_Toc145601481"^^xsd:anyURI ;
    dcat:theme legcons:Part .

F2021L00310:184 a legcons:Division,
        owl:Class,
        dcat:Resource ;
    rdfs:label "Division - D184 Division 3 Marks resembling official marks"@en-AU ;
    dct:hasPart F2021L00310:185,
        F2021L00310:186,
        F2021L00310:187 ;
    dct:isPartOf F2021L00310:159 ;
    dct:isReferencedBy F2021L00310: ;
    rdfs:comment "Division 3 Marks resembling official marks - Abrievated Graph Key: D184"@en-AU ;
    skos:broader F2021L00310:185,
        F2021L00310:186,
        F2021L00310:187 ;
    skos:definition "Division 3 Marks resembling official marks"@en-AU ;
    skos:narrower F2021L00310:159 ;
    skos:prefLabel "Division D184"@en-AU ;
    dcat:accessURL <https://www.legislation.gov.au/F2021L00310/2023-08-04/2023-08-04/text/1/epub/OEBPS/document_1/document_1.html#_Toc145601510> ;
    dcat:landingPage "https://www.legislation.gov.au/F2021L00310/2023-08-04/2023-08-04/text/1/epub/OEBPS/document_1/document_1.html#_Toc145601510"^^xsd:anyURI ;
    dcat:theme legcons:Division .

F2021L00310:195 a legcons:Chapter,
        owl:Class,
        dcat:Resource ;
    rdfs:label "Chapter - C195 Chapter 9 Powers and officials"@en-AU ;
    dct:hasPart F2021L00310:196,
        F2021L00310:216,
        F2021L00310:218,
        F2021L00310:220 ;
    dct:isReferencedBy F2021L00310: ;
    rdfs:comment "Chapter 9 Powers and officials - Abrievated Graph Key: C195"@en-AU ;
    skos:broader F2021L00310:196,
        F2021L00310:216,
        F2021L00310:218,
        F2021L00310:220 ;
    skos:definition "Chapter 9 Powers and officials"@en-AU ;
    skos:prefLabel "Chapter C195"@en-AU ;
    dcat:accessURL <https://www.legislation.gov.au/F2021L00310/2023-08-04/2023-08-04/text/1/epub/OEBPS/document_1/document_1.html#_Toc145601521> ;
    dcat:landingPage "https://www.legislation.gov.au/F2021L00310/2023-08-04/2023-08-04/text/1/epub/OEBPS/document_1/document_1.html#_Toc145601521"^^xsd:anyURI ;
    dcat:theme legcons:Chapter .

F2021L00310:196 a legcons:Part,
        owl:Class,
        dcat:Resource ;
    rdfs:label "Part - P196 Part 1 Audits"@en-AU ;
    dct:hasPart F2021L00310:197,
        F2021L00310:199,
        F2021L00310:204 ;
    dct:isPartOf F2021L00310:195 ;
    dct:isReferencedBy F2021L00310: ;
    rdfs:comment "Part 1 Audits - Abrievated Graph Key: P196"@en-AU ;
    skos:broader F2021L00310:197,
        F2021L00310:199,
        F2021L00310:204 ;
    skos:definition "Part 1 Audits"@en-AU ;
    skos:narrower F2021L00310:195 ;
    skos:prefLabel "Part P196"@en-AU ;
    dcat:accessURL <https://www.legislation.gov.au/F2021L00310/2023-08-04/2023-08-04/text/1/epub/OEBPS/document_1/document_1.html#_Toc145601522> ;
    dcat:landingPage "https://www.legislation.gov.au/F2021L00310/2023-08-04/2023-08-04/text/1/epub/OEBPS/document_1/document_1.html#_Toc145601522"^^xsd:anyURI ;
    dcat:theme legcons:Part .

F2021L00310:287 a legcons:Part,
        owl:Class,
        dcat:Resource ;
    rdfs:label "Part - P287 Part 4 Other matters relating to export"@en-AU ;
    dct:hasPart F2021L00310:288,
        F2021L00310:290,
        F2021L00310:293 ;
    dct:isPartOf F2021L00310:264 ;
    dct:isReferencedBy F2021L00310: ;
    rdfs:comment "Part 4 Other matters relating to export - Abrievated Graph Key: P287"@en-AU ;
    skos:broader F2021L00310:288,
        F2021L00310:290,
        F2021L00310:293 ;
    skos:definition "Part 4 Other matters relating to export"@en-AU ;
    skos:narrower F2021L00310:264 ;
    skos:prefLabel "Part P287"@en-AU ;
    dcat:accessURL <https://www.legislation.gov.au/F2021L00310/2023-08-04/2023-08-04/text/1/epub/OEBPS/document_1/document_1.html#_Toc145601613> ;
    dcat:landingPage "https://www.legislation.gov.au/F2021L00310/2023-08-04/2023-08-04/text/1/epub/OEBPS/document_1/document_1.html#_Toc145601613"^^xsd:anyURI ;
    dcat:theme legcons:Part .

F2021L00310:297 a legcons:Division,
        owl:Class,
        dcat:Resource ;
    rdfs:label "Division - D297 Division 1 Approved auditors"@en-AU ;
    dct:hasPart F2021L00310:298,
        F2021L00310:299,
        F2021L00310:300 ;
    dct:isPartOf F2021L00310:296 ;
    dct:isReferencedBy F2021L00310: ;
    rdfs:comment "Division 1 Approved auditors - Abrievated Graph Key: D297"@en-AU ;
    skos:broader F2021L00310:298,
        F2021L00310:299,
        F2021L00310:300 ;
    skos:definition "Division 1 Approved auditors"@en-AU ;
    skos:narrower F2021L00310:296 ;
    skos:prefLabel "Division D297"@en-AU ;
    dcat:accessURL <https://www.legislation.gov.au/F2021L00310/2023-08-04/2023-08-04/text/1/epub/OEBPS/document_1/document_1.html#_Toc145601623> ;
    dcat:landingPage "https://www.legislation.gov.au/F2021L00310/2023-08-04/2023-08-04/text/1/epub/OEBPS/document_1/document_1.html#_Toc145601623"^^xsd:anyURI ;
    dcat:theme legcons:Division .

F2021L00310:56 a legcons:Part,
        owl:Class,
        dcat:Resource ;
    rdfs:label "Part - P56 Part 5 Matters relating to applications"@en-AU ;
    dct:hasPart F2021L00310:57,
        F2021L00310:58,
        F2021L00310:59 ;
    dct:isPartOf F2021L00310:34 ;
    dct:isReferencedBy F2021L00310: ;
    rdfs:comment "Part 5 Matters relating to applications - Abrievated Graph Key: P56"@en-AU ;
    skos:broader F2021L00310:57,
        F2021L00310:58,
        F2021L00310:59 ;
    skos:definition "Part 5 Matters relating to applications"@en-AU ;
    skos:narrower F2021L00310:34 ;
    skos:prefLabel "Part P56"@en-AU ;
    dcat:accessURL <https://www.legislation.gov.au/F2021L00310/2023-08-04/2023-08-04/text/1/epub/OEBPS/document_1/document_1.html#_Toc145601382> ;
    dcat:landingPage "https://www.legislation.gov.au/F2021L00310/2023-08-04/2023-08-04/text/1/epub/OEBPS/document_1/document_1.html#_Toc145601382"^^xsd:anyURI ;
    dcat:theme legcons:Part .

F2021L00310:99 a legcons:Division,
        owl:Class,
        dcat:Resource ;
    rdfs:label "Division - D99 Division 4 Trade descriptions"@en-AU ;
    dct:hasPart F2021L00310:100,
        F2021L00310:101,
        F2021L00310:102 ;
    dct:isPartOf F2021L00310:80 ;
    dct:isReferencedBy F2021L00310: ;
    rdfs:comment "Division 4 Trade descriptions - Abrievated Graph Key: D99"@en-AU ;
    skos:broader F2021L00310:100,
        F2021L00310:101,
        F2021L00310:102 ;
    skos:definition "Division 4 Trade descriptions"@en-AU ;
    skos:narrower F2021L00310:80 ;
    skos:prefLabel "Division D99"@en-AU ;
    dcat:accessURL <https://www.legislation.gov.au/F2021L00310/2023-08-04/2023-08-04/text/1/epub/OEBPS/document_1/document_1.html#_Toc145601425> ;
    dcat:landingPage "https://www.legislation.gov.au/F2021L00310/2023-08-04/2023-08-04/text/1/epub/OEBPS/document_1/document_1.html#_Toc145601425"^^xsd:anyURI ;
    dcat:theme legcons:Division .

F2021L00310:103 a legcons:Division,
        owl:Class,
        dcat:Resource ;
    rdfs:label "Division - D103 Division 5 Official marks"@en-AU ;
    dct:hasPart F2021L00310:104,
        F2021L00310:105,
        F2021L00310:106,
        F2021L00310:107 ;
    dct:isPartOf F2021L00310:80 ;
    dct:isReferencedBy F2021L00310: ;
    rdfs:comment "Division 5 Official marks - Abrievated Graph Key: D103"@en-AU ;
    skos:broader F2021L00310:104,
        F2021L00310:105,
        F2021L00310:106,
        F2021L00310:107 ;
    skos:definition "Division 5 Official marks"@en-AU ;
    skos:narrower F2021L00310:80 ;
    skos:prefLabel "Division D103"@en-AU ;
    dcat:accessURL <https://www.legislation.gov.au/F2021L00310/2023-08-04/2023-08-04/text/1/epub/OEBPS/document_1/document_1.html#_Toc145601429> ;
    dcat:landingPage "https://www.legislation.gov.au/F2021L00310/2023-08-04/2023-08-04/text/1/epub/OEBPS/document_1/document_1.html#_Toc145601429"^^xsd:anyURI ;
    dcat:theme legcons:Division .

F2021L00310:120 a legcons:Division,
        owl:Class,
        dcat:Resource ;
    rdfs:label "Division - D120 Division 9 Management practicesexport operations"@en-AU ;
    dct:hasPart F2021L00310:121,
        F2021L00310:122,
        F2021L00310:123,
        F2021L00310:124 ;
    dct:isPartOf F2021L00310:80 ;
    dct:isReferencedBy F2021L00310: ;
    rdfs:comment "Division 9 Management practicesexport operations - Abrievated Graph Key: D120"@en-AU ;
    skos:broader F2021L00310:121,
        F2021L00310:122,
        F2021L00310:123,
        F2021L00310:124 ;
    skos:definition "Division 9 Management practicesexport operations"@en-AU ;
    skos:narrower F2021L00310:80 ;
    skos:prefLabel "Division D120"@en-AU ;
    dcat:accessURL <https://www.legislation.gov.au/F2021L00310/2023-08-04/2023-08-04/text/1/epub/OEBPS/document_1/document_1.html#_Toc145601446> ;
    dcat:landingPage "https://www.legislation.gov.au/F2021L00310/2023-08-04/2023-08-04/text/1/epub/OEBPS/document_1/document_1.html#_Toc145601446"^^xsd:anyURI ;
    dcat:theme legcons:Division .

F2021L00310:144 a legcons:Part,
        owl:Class,
        dcat:Resource ;
    rdfs:label "Part - P144 Part 3 Other matters"@en-AU ;
    dct:hasPart F2021L00310:145,
        F2021L00310:146,
        F2021L00310:147,
        F2021L00310:148 ;
    dct:isPartOf F2021L00310:137 ;
    dct:isReferencedBy F2021L00310: ;
    rdfs:comment "Part 3 Other matters - Abrievated Graph Key: P144"@en-AU ;
    skos:broader F2021L00310:145,
        F2021L00310:146,
        F2021L00310:147,
        F2021L00310:148 ;
    skos:definition "Part 3 Other matters"@en-AU ;
    skos:narrower F2021L00310:137 ;
    skos:prefLabel "Part P144"@en-AU ;
    dcat:accessURL <https://www.legislation.gov.au/F2021L00310/2023-08-04/2023-08-04/text/1/epub/OEBPS/document_1/document_1.html#_Toc145601470> ;
    dcat:landingPage "https://www.legislation.gov.au/F2021L00310/2023-08-04/2023-08-04/text/1/epub/OEBPS/document_1/document_1.html#_Toc145601470"^^xsd:anyURI ;
    dcat:theme legcons:Part .

F2021L00310:150 a legcons:Part,
        owl:Class,
        dcat:Resource ;
    rdfs:label "Part - P150 Part 1 Notices of intention to export"@en-AU ;
    dct:hasPart F2021L00310:151,
        F2021L00310:152,
        F2021L00310:153,
        F2021L00310:154 ;
    dct:isPartOf F2021L00310:149 ;
    dct:isReferencedBy F2021L00310: ;
    rdfs:comment "Part 1 Notices of intention to export - Abrievated Graph Key: P150"@en-AU ;
    skos:broader F2021L00310:151,
        F2021L00310:152,
        F2021L00310:153,
        F2021L00310:154 ;
    skos:definition "Part 1 Notices of intention to export"@en-AU ;
    skos:narrower F2021L00310:149 ;
    skos:prefLabel "Part P150"@en-AU ;
    dcat:accessURL <https://www.legislation.gov.au/F2021L00310/2023-08-04/2023-08-04/text/1/epub/OEBPS/document_1/document_1.html#_Toc145601476> ;
    dcat:landingPage "https://www.legislation.gov.au/F2021L00310/2023-08-04/2023-08-04/text/1/epub/OEBPS/document_1/document_1.html#_Toc145601476"^^xsd:anyURI ;
    dcat:theme legcons:Part .

F2021L00310:159 a legcons:Part,
        owl:Class,
        dcat:Resource ;
    rdfs:label "Part - P159 Part 3 Official marks"@en-AU ;
    dct:hasPart F2021L00310:160,
        F2021L00310:171,
        F2021L00310:184,
        F2021L00310:188 ;
    dct:isPartOf F2021L00310:149 ;
    dct:isReferencedBy F2021L00310: ;
    rdfs:comment "Part 3 Official marks - Abrievated Graph Key: P159"@en-AU ;
    skos:broader F2021L00310:160,
        F2021L00310:171,
        F2021L00310:184,
        F2021L00310:188 ;
    skos:definition "Part 3 Official marks"@en-AU ;
    skos:narrower F2021L00310:149 ;
    skos:prefLabel "Part P159"@en-AU ;
    dcat:accessURL <https://www.legislation.gov.au/F2021L00310/2023-08-04/2023-08-04/text/1/epub/OEBPS/document_1/document_1.html#_Toc145601485> ;
    dcat:landingPage "https://www.legislation.gov.au/F2021L00310/2023-08-04/2023-08-04/text/1/epub/OEBPS/document_1/document_1.html#_Toc145601485"^^xsd:anyURI ;
    dcat:theme legcons:Part .

F2021L00310:199 a legcons:Division,
        owl:Class,
        dcat:Resource ;
    rdfs:label "Division - D199 Division 2 Conduct of audit etc"@en-AU ;
    dct:hasPart F2021L00310:200,
        F2021L00310:201,
        F2021L00310:202,
        F2021L00310:203 ;
    dct:isPartOf F2021L00310:196 ;
    dct:isReferencedBy F2021L00310: ;
    rdfs:comment "Division 2 Conduct of audit etc - Abrievated Graph Key: D199"@en-AU ;
    skos:broader F2021L00310:200,
        F2021L00310:201,
        F2021L00310:202,
        F2021L00310:203 ;
    skos:definition "Division 2 Conduct of audit etc"@en-AU ;
    skos:narrower F2021L00310:196 ;
    skos:prefLabel "Division D199"@en-AU ;
    dcat:accessURL <https://www.legislation.gov.au/F2021L00310/2023-08-04/2023-08-04/text/1/epub/OEBPS/document_1/document_1.html#_Toc145601525> ;
    dcat:landingPage "https://www.legislation.gov.au/F2021L00310/2023-08-04/2023-08-04/text/1/epub/OEBPS/document_1/document_1.html#_Toc145601525"^^xsd:anyURI ;
    dcat:theme legcons:Division .

F2021L00310:220 a legcons:Part,
        owl:Class,
        dcat:Resource ;
    rdfs:label "Part - P220 Part 4 Authorised officers"@en-AU ;
    dct:hasPart F2021L00310:221,
        F2021L00310:223,
        F2021L00310:236,
        F2021L00310:238 ;
    dct:isPartOf F2021L00310:195 ;
    dct:isReferencedBy F2021L00310: ;
    rdfs:comment "Part 4 Authorised officers - Abrievated Graph Key: P220"@en-AU ;
    skos:broader F2021L00310:221,
        F2021L00310:223,
        F2021L00310:236,
        F2021L00310:238 ;
    skos:definition "Part 4 Authorised officers"@en-AU ;
    skos:narrower F2021L00310:195 ;
    skos:prefLabel "Part P220"@en-AU ;
    dcat:accessURL <https://www.legislation.gov.au/F2021L00310/2023-08-04/2023-08-04/text/1/epub/OEBPS/document_1/document_1.html#_Toc145601546> ;
    dcat:landingPage "https://www.legislation.gov.au/F2021L00310/2023-08-04/2023-08-04/text/1/epub/OEBPS/document_1/document_1.html#_Toc145601546"^^xsd:anyURI ;
    dcat:theme legcons:Part .

F2021L00310:243 a legcons:Chapter,
        owl:Class,
        dcat:Resource ;
    rdfs:label "Chapter - C243 Chapter 11 Miscellaneous"@en-AU ;
    dct:hasPart F2021L00310:244,
        F2021L00310:246,
        F2021L00310:257,
        F2021L00310:259,
        F2021L00310:262 ;
    dct:isReferencedBy F2021L00310: ;
    rdfs:comment "Chapter 11 Miscellaneous - Abrievated Graph Key: C243"@en-AU ;
    skos:broader F2021L00310:244,
        F2021L00310:246,
        F2021L00310:257,
        F2021L00310:259,
        F2021L00310:262 ;
    skos:definition "Chapter 11 Miscellaneous"@en-AU ;
    skos:prefLabel "Chapter C243"@en-AU ;
    dcat:accessURL <https://www.legislation.gov.au/F2021L00310/2023-08-04/2023-08-04/text/1/epub/OEBPS/document_1/document_1.html#_Toc145601569> ;
    dcat:landingPage "https://www.legislation.gov.au/F2021L00310/2023-08-04/2023-08-04/text/1/epub/OEBPS/document_1/document_1.html#_Toc145601569"^^xsd:anyURI ;
    dcat:theme legcons:Chapter .

F2021L00310:304 a legcons:Endnotes,
        owl:Class,
        dcat:Resource ;
    rdfs:label "Endnotes - E304 Endnotes"@en-AU ;
    dct:hasPart F2021L00310:305,
        F2021L00310:306,
        F2021L00310:307,
        F2021L00310:308 ;
    dct:isPartOf F2021L00310:264 ;
    dct:isReferencedBy F2021L00310: ;
    rdfs:comment "Endnotes - Abrievated Graph Key: E304"@en-AU ;
    skos:broader F2021L00310:305,
        F2021L00310:306,
        F2021L00310:307,
        F2021L00310:308 ;
    skos:definition "Endnotes"@en-AU ;
    skos:narrower F2021L00310:264 ;
    skos:prefLabel "Endnotes E304"@en-AU ;
    dcat:accessURL <https://www.legislation.gov.au/F2021L00310/2023-08-04/2023-08-04/text/1/epub/OEBPS/document_1/document_1.html#_Toc145601630> ;
    dcat:landingPage "https://www.legislation.gov.au/F2021L00310/2023-08-04/2023-08-04/text/1/epub/OEBPS/document_1/document_1.html#_Toc145601630"^^xsd:anyURI ;
    dcat:theme legcons:Endnotes .

F2021L00310:76 a legcons:Chapter,
        owl:Class,
        dcat:Resource ;
    rdfs:label "Chapter - C76 Chapter 5 Approved arrangements"@en-AU ;
    dct:hasPart F2021L00310:125,
        F2021L00310:127,
        F2021L00310:133,
        F2021L00310:77,
        F2021L00310:80 ;
    dct:isReferencedBy F2021L00310: ;
    rdfs:comment "Chapter 5 Approved arrangements - Abrievated Graph Key: C76"@en-AU ;
    skos:broader F2021L00310:125,
        F2021L00310:127,
        F2021L00310:133,
        F2021L00310:77,
        F2021L00310:80 ;
    skos:definition "Chapter 5 Approved arrangements"@en-AU ;
    skos:prefLabel "Chapter C76"@en-AU ;
    dcat:accessURL <https://www.legislation.gov.au/F2021L00310/2023-08-04/2023-08-04/text/1/epub/OEBPS/document_1/document_1.html#_Toc145601402> ;
    dcat:landingPage "https://www.legislation.gov.au/F2021L00310/2023-08-04/2023-08-04/text/1/epub/OEBPS/document_1/document_1.html#_Toc145601402"^^xsd:anyURI ;
    dcat:theme legcons:Chapter .

F2021L00310:264 a legcons:Chapter,
        owl:Class,
        dcat:Resource ;
    rdfs:label "Chapter - C264 Chapter 12 Transitional provisions"@en-AU ;
    dct:hasPart F2021L00310:265,
        F2021L00310:267,
        F2021L00310:285,
        F2021L00310:287,
        F2021L00310:296,
        F2021L00310:304 ;
    dct:isReferencedBy F2021L00310: ;
    rdfs:comment "Chapter 12 Transitional provisions - Abrievated Graph Key: C264"@en-AU ;
    skos:broader F2021L00310:265,
        F2021L00310:267,
        F2021L00310:285,
        F2021L00310:287,
        F2021L00310:296,
        F2021L00310:304 ;
    skos:definition "Chapter 12 Transitional provisions"@en-AU ;
    skos:prefLabel "Chapter C264"@en-AU ;
    dcat:accessURL <https://www.legislation.gov.au/F2021L00310/2023-08-04/2023-08-04/text/1/epub/OEBPS/document_1/document_1.html#_Toc145601590> ;
    dcat:landingPage "https://www.legislation.gov.au/F2021L00310/2023-08-04/2023-08-04/text/1/epub/OEBPS/document_1/document_1.html#_Toc145601590"^^xsd:anyURI ;
    dcat:theme legcons:Chapter .

F2021L00310:28 a legcons:Part,
        owl:Class,
        dcat:Resource ;
    rdfs:label "Part - P28 Part 3 Government certificates"@en-AU ;
    dct:hasPart F2021L00310:29,
        F2021L00310:30,
        F2021L00310:31,
        F2021L00310:32,
        F2021L00310:33 ;
    dct:isPartOf F2021L00310:13 ;
    dct:isReferencedBy F2021L00310: ;
    rdfs:comment "Part 3 Government certificates - Abrievated Graph Key: P28"@en-AU ;
    skos:broader F2021L00310:29,
        F2021L00310:30,
        F2021L00310:31,
        F2021L00310:32,
        F2021L00310:33 ;
    skos:definition "Part 3 Government certificates"@en-AU ;
    skos:narrower F2021L00310:13 ;
    skos:prefLabel "Part P28"@en-AU ;
    dcat:accessURL <https://www.legislation.gov.au/F2021L00310/2023-08-04/2023-08-04/text/1/epub/OEBPS/document_1/document_1.html#_Toc145601354> ;
    dcat:landingPage "https://www.legislation.gov.au/F2021L00310/2023-08-04/2023-08-04/text/1/epub/OEBPS/document_1/document_1.html#_Toc145601354"^^xsd:anyURI ;
    dcat:theme legcons:Part .

F2021L00310:34 a legcons:Chapter,
        owl:Class,
        dcat:Resource ;
    rdfs:label "Chapter - C34 Chapter 4 Registered establishments"@en-AU ;
    dct:hasPart F2021L00310:35,
        F2021L00310:44,
        F2021L00310:51,
        F2021L00310:54,
        F2021L00310:56,
        F2021L00310:60 ;
    dct:isReferencedBy F2021L00310: ;
    rdfs:comment "Chapter 4 Registered establishments - Abrievated Graph Key: C34"@en-AU ;
    skos:broader F2021L00310:35,
        F2021L00310:44,
        F2021L00310:51,
        F2021L00310:54,
        F2021L00310:56,
        F2021L00310:60 ;
    skos:definition "Chapter 4 Registered establishments"@en-AU ;
    skos:prefLabel "Chapter C34"@en-AU ;
    dcat:accessURL <https://www.legislation.gov.au/F2021L00310/2023-08-04/2023-08-04/text/1/epub/OEBPS/document_1/document_1.html#_Toc145601360> ;
    dcat:landingPage "https://www.legislation.gov.au/F2021L00310/2023-08-04/2023-08-04/text/1/epub/OEBPS/document_1/document_1.html#_Toc145601360"^^xsd:anyURI ;
    dcat:theme legcons:Chapter .

F2021L00310:70 a legcons:Division,
        owl:Class,
        dcat:Resource ;
    rdfs:label "Division - D70 Division 2 Variation of meat inspection services"@en-AU ;
    dct:hasPart F2021L00310:71,
        F2021L00310:72,
        F2021L00310:73,
        F2021L00310:74,
        F2021L00310:75 ;
    dct:isPartOf F2021L00310:60 ;
    dct:isReferencedBy F2021L00310: ;
    rdfs:comment "Division 2 Variation of meat inspection services - Abrievated Graph Key: D70"@en-AU ;
    skos:broader F2021L00310:71,
        F2021L00310:72,
        F2021L00310:73,
        F2021L00310:74,
        F2021L00310:75 ;
    skos:definition "Division 2 Variation of meat inspection services"@en-AU ;
    skos:narrower F2021L00310:60 ;
    skos:prefLabel "Division D70"@en-AU ;
    dcat:accessURL <https://www.legislation.gov.au/F2021L00310/2023-08-04/2023-08-04/text/1/epub/OEBPS/document_1/document_1.html#_Toc145601396> ;
    dcat:landingPage "https://www.legislation.gov.au/F2021L00310/2023-08-04/2023-08-04/text/1/epub/OEBPS/document_1/document_1.html#_Toc145601396"^^xsd:anyURI ;
    dcat:theme legcons:Division .

F2021L00310:108 a legcons:Division,
        owl:Class,
        dcat:Resource ;
    rdfs:label "Division - D108 Division 6 Segregation identification security traceability and integrity"@en-AU ;
    dct:hasPart F2021L00310:109,
        F2021L00310:110,
        F2021L00310:111,
        F2021L00310:112,
        F2021L00310:113,
        F2021L00310:114 ;
    dct:isPartOf F2021L00310:80 ;
    dct:isReferencedBy F2021L00310: ;
    rdfs:comment "Division 6 Segregation identification security traceability and integrity - Abrievated Graph Key: D108"@en-AU ;
    skos:broader F2021L00310:109,
        F2021L00310:110,
        F2021L00310:111,
        F2021L00310:112,
        F2021L00310:113,
        F2021L00310:114 ;
    skos:definition "Division 6 Segregation identification security traceability and integrity"@en-AU ;
    skos:narrower F2021L00310:80 ;
    skos:prefLabel "Division D108"@en-AU ;
    dcat:accessURL <https://www.legislation.gov.au/F2021L00310/2023-08-04/2023-08-04/text/1/epub/OEBPS/document_1/document_1.html#_Toc145601434> ;
    dcat:landingPage "https://www.legislation.gov.au/F2021L00310/2023-08-04/2023-08-04/text/1/epub/OEBPS/document_1/document_1.html#_Toc145601434"^^xsd:anyURI ;
    dcat:theme legcons:Division .

F2021L00310:188 a legcons:Division,
        owl:Class,
        dcat:Resource ;
    rdfs:label "Division - D188 Division 4 Official marking devices"@en-AU ;
    dct:hasPart F2021L00310:189,
        F2021L00310:190,
        F2021L00310:191,
        F2021L00310:192,
        F2021L00310:193,
        F2021L00310:194 ;
    dct:isPartOf F2021L00310:159 ;
    dct:isReferencedBy F2021L00310: ;
    rdfs:comment "Division 4 Official marking devices - Abrievated Graph Key: D188"@en-AU ;
    skos:broader F2021L00310:189,
        F2021L00310:190,
        F2021L00310:191,
        F2021L00310:192,
        F2021L00310:193,
        F2021L00310:194 ;
    skos:definition "Division 4 Official marking devices"@en-AU ;
    skos:narrower F2021L00310:159 ;
    skos:prefLabel "Division D188"@en-AU ;
    dcat:accessURL <https://www.legislation.gov.au/F2021L00310/2023-08-04/2023-08-04/text/1/epub/OEBPS/document_1/document_1.html#_Toc145601514> ;
    dcat:landingPage "https://www.legislation.gov.au/F2021L00310/2023-08-04/2023-08-04/text/1/epub/OEBPS/document_1/document_1.html#_Toc145601514"^^xsd:anyURI ;
    dcat:theme legcons:Division .

F2021L00310:21 a legcons:Part,
        owl:Class,
        dcat:Resource ;
    rdfs:label "Part - P21 Part 2 Exemptions"@en-AU ;
    dct:hasPart F2021L00310:22,
        F2021L00310:23,
        F2021L00310:24,
        F2021L00310:25,
        F2021L00310:26,
        F2021L00310:27 ;
    dct:isPartOf F2021L00310:13 ;
    dct:isReferencedBy F2021L00310: ;
    rdfs:comment "Part 2 Exemptions - Abrievated Graph Key: P21"@en-AU ;
    skos:broader F2021L00310:22,
        F2021L00310:23,
        F2021L00310:24,
        F2021L00310:25,
        F2021L00310:26,
        F2021L00310:27 ;
    skos:definition "Part 2 Exemptions"@en-AU ;
    skos:narrower F2021L00310:13 ;
    skos:prefLabel "Part P21"@en-AU ;
    dcat:accessURL <https://www.legislation.gov.au/F2021L00310/2023-08-04/2023-08-04/text/1/epub/OEBPS/document_1/document_1.html#_Toc145601347> ;
    dcat:landingPage "https://www.legislation.gov.au/F2021L00310/2023-08-04/2023-08-04/text/1/epub/OEBPS/document_1/document_1.html#_Toc145601347"^^xsd:anyURI ;
    dcat:theme legcons:Part .

F2021L00310:44 a legcons:Part,
        owl:Class,
        dcat:Resource ;
    rdfs:label "Part - P44 Part 2 Conditions of registration"@en-AU ;
    dct:hasPart F2021L00310:45,
        F2021L00310:46,
        F2021L00310:47,
        F2021L00310:48,
        F2021L00310:49,
        F2021L00310:50 ;
    dct:isPartOf F2021L00310:34 ;
    dct:isReferencedBy F2021L00310: ;
    rdfs:comment "Part 2 Conditions of registration - Abrievated Graph Key: P44"@en-AU ;
    skos:broader F2021L00310:45,
        F2021L00310:46,
        F2021L00310:47,
        F2021L00310:48,
        F2021L00310:49,
        F2021L00310:50 ;
    skos:definition "Part 2 Conditions of registration"@en-AU ;
    skos:narrower F2021L00310:34 ;
    skos:prefLabel "Part P44"@en-AU ;
    dcat:accessURL <https://www.legislation.gov.au/F2021L00310/2023-08-04/2023-08-04/text/1/epub/OEBPS/document_1/document_1.html#_Toc145601370> ;
    dcat:landingPage "https://www.legislation.gov.au/F2021L00310/2023-08-04/2023-08-04/text/1/epub/OEBPS/document_1/document_1.html#_Toc145601370"^^xsd:anyURI ;
    dcat:theme legcons:Part .

F2021L00310:35 a legcons:Part,
        owl:Class,
        dcat:Resource ;
    rdfs:label "Part - P35 Part 1 Requirements for registration"@en-AU ;
    dct:hasPart F2021L00310:36,
        F2021L00310:37,
        F2021L00310:38,
        F2021L00310:39,
        F2021L00310:40,
        F2021L00310:41,
        F2021L00310:42,
        F2021L00310:43 ;
    dct:isPartOf F2021L00310:34 ;
    dct:isReferencedBy F2021L00310: ;
    rdfs:comment "Part 1 Requirements for registration - Abrievated Graph Key: P35"@en-AU ;
    skos:broader F2021L00310:36,
        F2021L00310:37,
        F2021L00310:38,
        F2021L00310:39,
        F2021L00310:40,
        F2021L00310:41,
        F2021L00310:42,
        F2021L00310:43 ;
    skos:definition "Part 1 Requirements for registration"@en-AU ;
    skos:narrower F2021L00310:34 ;
    skos:prefLabel "Part P35"@en-AU ;
    dcat:accessURL <https://www.legislation.gov.au/F2021L00310/2023-08-04/2023-08-04/text/1/epub/OEBPS/document_1/document_1.html#_Toc145601361> ;
    dcat:landingPage "https://www.legislation.gov.au/F2021L00310/2023-08-04/2023-08-04/text/1/epub/OEBPS/document_1/document_1.html#_Toc145601361"^^xsd:anyURI ;
    dcat:theme legcons:Part .

F2021L00310:61 a legcons:Division,
        owl:Class,
        dcat:Resource ;
    rdfs:label "Division - D61 Division 1 Allocation of meat inspection services"@en-AU ;
    dct:hasPart F2021L00310:62,
        F2021L00310:63,
        F2021L00310:64,
        F2021L00310:65,
        F2021L00310:66,
        F2021L00310:67,
        F2021L00310:68,
        F2021L00310:69 ;
    dct:isPartOf F2021L00310:60 ;
    dct:isReferencedBy F2021L00310: ;
    rdfs:comment "Division 1 Allocation of meat inspection services - Abrievated Graph Key: D61"@en-AU ;
    skos:broader F2021L00310:62,
        F2021L00310:63,
        F2021L00310:64,
        F2021L00310:65,
        F2021L00310:66,
        F2021L00310:67,
        F2021L00310:68,
        F2021L00310:69 ;
    skos:definition "Division 1 Allocation of meat inspection services"@en-AU ;
    skos:narrower F2021L00310:60 ;
    skos:prefLabel "Division D61"@en-AU ;
    dcat:accessURL <https://www.legislation.gov.au/F2021L00310/2023-08-04/2023-08-04/text/1/epub/OEBPS/document_1/document_1.html#_Toc145601387> ;
    dcat:landingPage "https://www.legislation.gov.au/F2021L00310/2023-08-04/2023-08-04/text/1/epub/OEBPS/document_1/document_1.html#_Toc145601387"^^xsd:anyURI ;
    dcat:theme legcons:Division .

F2021L00310:80 a legcons:Part,
        owl:Class,
        dcat:Resource ;
    rdfs:label "Part - P80 Part 2 Conditions of approved arrangement"@en-AU ;
    dct:hasPart F2021L00310:103,
        F2021L00310:108,
        F2021L00310:115,
        F2021L00310:118,
        F2021L00310:120,
        F2021L00310:81,
        F2021L00310:83,
        F2021L00310:86,
        F2021L00310:99 ;
    dct:isPartOf F2021L00310:76 ;
    dct:isReferencedBy F2021L00310: ;
    rdfs:comment "Part 2 Conditions of approved arrangement - Abrievated Graph Key: P80"@en-AU ;
    skos:broader F2021L00310:103,
        F2021L00310:108,
        F2021L00310:115,
        F2021L00310:118,
        F2021L00310:120,
        F2021L00310:81,
        F2021L00310:83,
        F2021L00310:86,
        F2021L00310:99 ;
    skos:definition "Part 2 Conditions of approved arrangement"@en-AU ;
    skos:narrower F2021L00310:76 ;
    skos:prefLabel "Part P80"@en-AU ;
    dcat:accessURL <https://www.legislation.gov.au/F2021L00310/2023-08-04/2023-08-04/text/1/epub/OEBPS/document_1/document_1.html#_Toc145601406> ;
    dcat:landingPage "https://www.legislation.gov.au/F2021L00310/2023-08-04/2023-08-04/text/1/epub/OEBPS/document_1/document_1.html#_Toc145601406"^^xsd:anyURI ;
    dcat:theme legcons:Part .

F2021L00310:1 a legcons:Chapter,
        owl:Class,
        dcat:Resource ;
    rdfs:label "Chapter - C1 Chapter 1 Preliminary"@en-AU ;
    dct:hasPart F2021L00310:10,
        F2021L00310:11,
        F2021L00310:12,
        F2021L00310:2,
        F2021L00310:3,
        F2021L00310:4,
        F2021L00310:5,
        F2021L00310:6,
        F2021L00310:7,
        F2021L00310:8,
        F2021L00310:9 ;
    dct:isReferencedBy F2021L00310: ;
    rdfs:comment "Chapter 1 Preliminary - Abrievated Graph Key: C1"@en-AU ;
    skos:broader F2021L00310:10,
        F2021L00310:11,
        F2021L00310:12,
        F2021L00310:2,
        F2021L00310:3,
        F2021L00310:4,
        F2021L00310:5,
        F2021L00310:6,
        F2021L00310:7,
        F2021L00310:8,
        F2021L00310:9 ;
    skos:definition "Chapter 1 Preliminary"@en-AU ;
    skos:prefLabel "Chapter C1"@en-AU ;
    dcat:accessURL <https://www.legislation.gov.au/F2021L00310/2023-08-04/2023-08-04/text/1/epub/OEBPS/document_1/document_1.html#_Toc145601327> ;
    dcat:landingPage "https://www.legislation.gov.au/F2021L00310/2023-08-04/2023-08-04/text/1/epub/OEBPS/document_1/document_1.html#_Toc145601327"^^xsd:anyURI ;
    dcat:theme legcons:Chapter .

F2021L00310:160 a legcons:Division,
        owl:Class,
        dcat:Resource ;
    rdfs:label "Division - D160 Division 1 Marks that are official marks"@en-AU ;
    dct:hasPart F2021L00310:161,
        F2021L00310:162,
        F2021L00310:163,
        F2021L00310:164,
        F2021L00310:165,
        F2021L00310:166,
        F2021L00310:167,
        F2021L00310:168,
        F2021L00310:169,
        F2021L00310:170 ;
    dct:isPartOf F2021L00310:159 ;
    dct:isReferencedBy F2021L00310: ;
    rdfs:comment "Division 1 Marks that are official marks - Abrievated Graph Key: D160"@en-AU ;
    skos:broader F2021L00310:161,
        F2021L00310:162,
        F2021L00310:163,
        F2021L00310:164,
        F2021L00310:165,
        F2021L00310:166,
        F2021L00310:167,
        F2021L00310:168,
        F2021L00310:169,
        F2021L00310:170 ;
    skos:definition "Division 1 Marks that are official marks"@en-AU ;
    skos:narrower F2021L00310:159 ;
    skos:prefLabel "Division D160"@en-AU ;
    dcat:accessURL <https://www.legislation.gov.au/F2021L00310/2023-08-04/2023-08-04/text/1/epub/OEBPS/document_1/document_1.html#_Toc145601486> ;
    dcat:landingPage "https://www.legislation.gov.au/F2021L00310/2023-08-04/2023-08-04/text/1/epub/OEBPS/document_1/document_1.html#_Toc145601486"^^xsd:anyURI ;
    dcat:theme legcons:Division .

F2021L00310:246 a legcons:Part,
        owl:Class,
        dcat:Resource ;
    rdfs:label "Part - P246 Part 2 Records"@en-AU ;
    dct:hasPart F2021L00310:247,
        F2021L00310:248,
        F2021L00310:249,
        F2021L00310:250,
        F2021L00310:251,
        F2021L00310:252,
        F2021L00310:253,
        F2021L00310:254,
        F2021L00310:255,
        F2021L00310:256 ;
    dct:isPartOf F2021L00310:243 ;
    dct:isReferencedBy F2021L00310: ;
    rdfs:comment "Part 2 Records - Abrievated Graph Key: P246"@en-AU ;
    skos:broader F2021L00310:247,
        F2021L00310:248,
        F2021L00310:249,
        F2021L00310:250,
        F2021L00310:251,
        F2021L00310:252,
        F2021L00310:253,
        F2021L00310:254,
        F2021L00310:255,
        F2021L00310:256 ;
    skos:definition "Part 2 Records"@en-AU ;
    skos:narrower F2021L00310:243 ;
    skos:prefLabel "Part P246"@en-AU ;
    dcat:accessURL <https://www.legislation.gov.au/F2021L00310/2023-08-04/2023-08-04/text/1/epub/OEBPS/document_1/document_1.html#_Toc145601572> ;
    dcat:landingPage "https://www.legislation.gov.au/F2021L00310/2023-08-04/2023-08-04/text/1/epub/OEBPS/document_1/document_1.html#_Toc145601572"^^xsd:anyURI ;
    dcat:theme legcons:Part .

F2021L00310:204 a legcons:Division,
        owl:Class,
        dcat:Resource ;
    rdfs:label "Division - D204 Division 3 Approved auditors"@en-AU ;
    dct:hasPart F2021L00310:205,
        F2021L00310:206,
        F2021L00310:207,
        F2021L00310:208,
        F2021L00310:209,
        F2021L00310:210,
        F2021L00310:211,
        F2021L00310:212,
        F2021L00310:213,
        F2021L00310:214,
        F2021L00310:215 ;
    dct:isPartOf F2021L00310:196 ;
    dct:isReferencedBy F2021L00310: ;
    rdfs:comment "Division 3 Approved auditors - Abrievated Graph Key: D204"@en-AU ;
    skos:broader F2021L00310:205,
        F2021L00310:206,
        F2021L00310:207,
        F2021L00310:208,
        F2021L00310:209,
        F2021L00310:210,
        F2021L00310:211,
        F2021L00310:212,
        F2021L00310:213,
        F2021L00310:214,
        F2021L00310:215 ;
    skos:definition "Division 3 Approved auditors"@en-AU ;
    skos:narrower F2021L00310:196 ;
    skos:prefLabel "Division D204"@en-AU ;
    dcat:accessURL <https://www.legislation.gov.au/F2021L00310/2023-08-04/2023-08-04/text/1/epub/OEBPS/document_1/document_1.html#_Toc145601530> ;
    dcat:landingPage "https://www.legislation.gov.au/F2021L00310/2023-08-04/2023-08-04/text/1/epub/OEBPS/document_1/document_1.html#_Toc145601530"^^xsd:anyURI ;
    dcat:theme legcons:Division .

F2021L00310:171 a legcons:Division,
        owl:Class,
        dcat:Resource ;
    rdfs:label "Division - D171 Division 2 General rules relating to official marks"@en-AU ;
    dct:hasPart F2021L00310:172,
        F2021L00310:173,
        F2021L00310:174,
        F2021L00310:175,
        F2021L00310:176,
        F2021L00310:177,
        F2021L00310:178,
        F2021L00310:179,
        F2021L00310:180,
        F2021L00310:181,
        F2021L00310:182,
        F2021L00310:183 ;
    dct:isPartOf F2021L00310:159 ;
    dct:isReferencedBy F2021L00310: ;
    rdfs:comment "Division 2 General rules relating to official marks - Abrievated Graph Key: D171"@en-AU ;
    skos:broader F2021L00310:172,
        F2021L00310:173,
        F2021L00310:174,
        F2021L00310:175,
        F2021L00310:176,
        F2021L00310:177,
        F2021L00310:178,
        F2021L00310:179,
        F2021L00310:180,
        F2021L00310:181,
        F2021L00310:182,
        F2021L00310:183 ;
    skos:definition "Division 2 General rules relating to official marks"@en-AU ;
    skos:narrower F2021L00310:159 ;
    skos:prefLabel "Division D171"@en-AU ;
    dcat:accessURL <https://www.legislation.gov.au/F2021L00310/2023-08-04/2023-08-04/text/1/epub/OEBPS/document_1/document_1.html#_Toc145601497> ;
    dcat:landingPage "https://www.legislation.gov.au/F2021L00310/2023-08-04/2023-08-04/text/1/epub/OEBPS/document_1/document_1.html#_Toc145601497"^^xsd:anyURI ;
    dcat:theme legcons:Division .

F2021L00310:223 a legcons:Division,
        owl:Class,
        dcat:Resource ;
    rdfs:label "Division - D223 Division 2 Functions and powers"@en-AU ;
    dct:hasPart F2021L00310:224,
        F2021L00310:225,
        F2021L00310:226,
        F2021L00310:227,
        F2021L00310:228,
        F2021L00310:229,
        F2021L00310:230,
        F2021L00310:231,
        F2021L00310:232,
        F2021L00310:233,
        F2021L00310:234,
        F2021L00310:235 ;
    dct:isPartOf F2021L00310:220 ;
    dct:isReferencedBy F2021L00310: ;
    rdfs:comment "Division 2 Functions and powers - Abrievated Graph Key: D223"@en-AU ;
    skos:broader F2021L00310:224,
        F2021L00310:225,
        F2021L00310:226,
        F2021L00310:227,
        F2021L00310:228,
        F2021L00310:229,
        F2021L00310:230,
        F2021L00310:231,
        F2021L00310:232,
        F2021L00310:233,
        F2021L00310:234,
        F2021L00310:235 ;
    skos:definition "Division 2 Functions and powers"@en-AU ;
    skos:narrower F2021L00310:220 ;
    skos:prefLabel "Division D223"@en-AU ;
    dcat:accessURL <https://www.legislation.gov.au/F2021L00310/2023-08-04/2023-08-04/text/1/epub/OEBPS/document_1/document_1.html#_Toc145601549> ;
    dcat:landingPage "https://www.legislation.gov.au/F2021L00310/2023-08-04/2023-08-04/text/1/epub/OEBPS/document_1/document_1.html#_Toc145601549"^^xsd:anyURI ;
    dcat:theme legcons:Division .

F2021L00310:86 a legcons:Division,
        owl:Class,
        dcat:Resource ;
    rdfs:label "Division - D86 Division 3 Preparation and transport"@en-AU ;
    dct:hasPart F2021L00310:87,
        F2021L00310:88,
        F2021L00310:89,
        F2021L00310:90,
        F2021L00310:91,
        F2021L00310:92,
        F2021L00310:93,
        F2021L00310:94,
        F2021L00310:95,
        F2021L00310:96,
        F2021L00310:97,
        F2021L00310:98 ;
    dct:isPartOf F2021L00310:80 ;
    dct:isReferencedBy F2021L00310: ;
    rdfs:comment "Division 3 Preparation and transport - Abrievated Graph Key: D86"@en-AU ;
    skos:broader F2021L00310:87,
        F2021L00310:88,
        F2021L00310:89,
        F2021L00310:90,
        F2021L00310:91,
        F2021L00310:92,
        F2021L00310:93,
        F2021L00310:94,
        F2021L00310:95,
        F2021L00310:96,
        F2021L00310:97,
        F2021L00310:98 ;
    skos:definition "Division 3 Preparation and transport"@en-AU ;
    skos:narrower F2021L00310:80 ;
    skos:prefLabel "Division D86"@en-AU ;
    dcat:accessURL <https://www.legislation.gov.au/F2021L00310/2023-08-04/2023-08-04/text/1/epub/OEBPS/document_1/document_1.html#_Toc145601412> ;
    dcat:landingPage "https://www.legislation.gov.au/F2021L00310/2023-08-04/2023-08-04/text/1/epub/OEBPS/document_1/document_1.html#_Toc145601412"^^xsd:anyURI ;
    dcat:theme legcons:Division .

F2021L00310:267 a legcons:Part,
        owl:Class,
        dcat:Resource ;
    rdfs:label "Part - P267 Part 2 Registered establishments meat inspection services"@en-AU ;
    dct:hasPart F2021L00310:268,
        F2021L00310:269,
        F2021L00310:270,
        F2021L00310:271,
        F2021L00310:272,
        F2021L00310:273,
        F2021L00310:274,
        F2021L00310:275,
        F2021L00310:276,
        F2021L00310:277,
        F2021L00310:278,
        F2021L00310:279,
        F2021L00310:280,
        F2021L00310:281,
        F2021L00310:282,
        F2021L00310:283,
        F2021L00310:284 ;
    dct:isPartOf F2021L00310:264 ;
    dct:isReferencedBy F2021L00310: ;
    rdfs:comment "Part 2 Registered establishments meat inspection services - Abrievated Graph Key: P267"@en-AU ;
    skos:broader F2021L00310:268,
        F2021L00310:269,
        F2021L00310:270,
        F2021L00310:271,
        F2021L00310:272,
        F2021L00310:273,
        F2021L00310:274,
        F2021L00310:275,
        F2021L00310:276,
        F2021L00310:277,
        F2021L00310:278,
        F2021L00310:279,
        F2021L00310:280,
        F2021L00310:281,
        F2021L00310:282,
        F2021L00310:283,
        F2021L00310:284 ;
    skos:definition "Part 2 Registered establishments meat inspection services"@en-AU ;
    skos:narrower F2021L00310:264 ;
    skos:prefLabel "Part P267"@en-AU ;
    dcat:accessURL <https://www.legislation.gov.au/F2021L00310/2023-08-04/2023-08-04/text/1/epub/OEBPS/document_1/document_1.html#_Toc145601593> ;
    dcat:landingPage "https://www.legislation.gov.au/F2021L00310/2023-08-04/2023-08-04/text/1/epub/OEBPS/document_1/document_1.html#_Toc145601593"^^xsd:anyURI ;
    dcat:theme legcons:Part .

F2021L00310: a owl:Class,
        dcat:Dataset,
        dcat:Resource ;
    rdfs:label "Export Control (Poultry Meat and Poultry Meat Products) Rules 2021" ;
    dct:Jurisdiction " Department of Agriculture, Fisheries and Forestry "@en-AU ;
    dct:created "2024-08-30T15:13:59.580379"^^xsd:dateTime ;
    dct:creator "https://orcid.org/0009-0007-8434-7325"^^xsd:anyURI ;
    dct:date "2023-08-04T00:00:00+10:00"^^xsd:dateTime ;
    dct:description "Export Control (Poultry Meat and Poultry Meat Products) Rules 2021"@en-AU ;
    dct:identifier "https://www.legislation.gov.au/F2021L00310/latest"^^xsd:anyURI ;
    dct:license <https://creativecommons.org/licenses/by-sa/4.0/> ;
    dct:source "scheme=AGLSTERMS.AglsAgent; corporateName=Office Parliamentary Counsel; address=Locked Bag 30 Kingston ACT 2604; contact=+61 2 6120 1400"@en-AU ;
    dct:subject "Export Control (Poultry Meat and Poultry Meat Products) Rules 2021"@en-AU ;
    dct:title "Export Control (Poultry Meat and Poultry Meat Products) Rules 2021"@en-AU ;
    owl:imports legcons: ;
    dcat:theme legcons:Chapter,
        legcons:Division,
        legcons:Endnotes,
        legcons:Item,
        legcons:Part ;
    schema:identifier "F2021L00310" ;
    schema:status "In force" ;
    schema:version "F2023C00777 (C02)" .

