@prefix F2021L00312: <http://example.org/au/leg/dataset/F2021L00312/> .
@prefix dcat: <http://www.w3.org/ns/dcat#> .
@prefix dct: <http://purl.org/dc/terms/> .
@prefix legcons: <http://example.org/au/leg/concepts/> .
@prefix owl: <http://www.w3.org/2002/07/owl#> .
@prefix rdfs: <http://www.w3.org/2000/01/rdf-schema#> .
@prefix schema: <https://schema.org/> .
@prefix skos: <http://www.w3.org/2004/02/skos/core#> .
@prefix xsd: <http://www.w3.org/2001/XMLSchema#> .

F2021L00312:100 a legcons:Item,
        owl:Class,
        dcat:Resource ;
    rdfs:label "Item - I100 5 30  Labelling and naming of ingredients"@en-AU ;
    dct:isPartOf F2021L00312:97 ;
    dct:isReferencedBy F2021L00312: ;
    rdfs:comment "5 30  Labelling and naming of ingredients - Abrievated Graph Key: I100"@en-AU ;
    skos:definition "5 30  Labelling and naming of ingredients"@en-AU ;
    skos:narrower F2021L00312:97 ;
    skos:prefLabel "Item I100"@en-AU ;
    dcat:accessURL <https://www.legislation.gov.au/F2021L00312/asmade/2021-03-24/text/original/epub/OEBPS/document_1/document_1.html#_Toc65843384> ;
    dcat:landingPage "https://www.legislation.gov.au/F2021L00312/asmade/2021-03-24/text/original/epub/OEBPS/document_1/document_1.html#_Toc65843384"^^xsd:anyURI ;
    dcat:theme legcons:Item .

F2021L00312:101 a legcons:Item,
        owl:Class,
        dcat:Resource ;
    rdfs:label "Item - I101 5 31  Trade descriptions applied to packaging etc"@en-AU ;
    dct:isPartOf F2021L00312:97 ;
    dct:isReferencedBy F2021L00312: ;
    rdfs:comment "5 31  Trade descriptions applied to packaging etc - Abrievated Graph Key: I101"@en-AU ;
    skos:definition "5 31  Trade descriptions applied to packaging etc"@en-AU ;
    skos:narrower F2021L00312:97 ;
    skos:prefLabel "Item I101"@en-AU ;
    dcat:accessURL <https://www.legislation.gov.au/F2021L00312/asmade/2021-03-24/text/original/epub/OEBPS/document_1/document_1.html#_Toc65843385> ;
    dcat:landingPage "https://www.legislation.gov.au/F2021L00312/asmade/2021-03-24/text/original/epub/OEBPS/document_1/document_1.html#_Toc65843385"^^xsd:anyURI ;
    dcat:theme legcons:Item .

F2021L00312:103 a legcons:Item,
        owl:Class,
        dcat:Resource ;
    rdfs:label "Item - I103 5 32  Alteration of or interference with official mark"@en-AU ;
    dct:isPartOf F2021L00312:102 ;
    dct:isReferencedBy F2021L00312: ;
    rdfs:comment "5 32  Alteration of or interference with official mark - Abrievated Graph Key: I103"@en-AU ;
    skos:definition "5 32  Alteration of or interference with official mark"@en-AU ;
    skos:narrower F2021L00312:102 ;
    skos:prefLabel "Item I103"@en-AU ;
    dcat:accessURL <https://www.legislation.gov.au/F2021L00312/asmade/2021-03-24/text/original/epub/OEBPS/document_1/document_1.html#_Toc65843387> ;
    dcat:landingPage "https://www.legislation.gov.au/F2021L00312/asmade/2021-03-24/text/original/epub/OEBPS/document_1/document_1.html#_Toc65843387"^^xsd:anyURI ;
    dcat:theme legcons:Item .

F2021L00312:105 a legcons:Item,
        owl:Class,
        dcat:Resource ;
    rdfs:label "Item - I105 5 33  Segregation identification and traceabilitygeneral"@en-AU ;
    dct:isPartOf F2021L00312:104 ;
    dct:isReferencedBy F2021L00312: ;
    rdfs:comment "5 33  Segregation identification and traceabilitygeneral - Abrievated Graph Key: I105"@en-AU ;
    skos:definition "5 33  Segregation identification and traceabilitygeneral"@en-AU ;
    skos:narrower F2021L00312:104 ;
    skos:prefLabel "Item I105"@en-AU ;
    dcat:accessURL <https://www.legislation.gov.au/F2021L00312/asmade/2021-03-24/text/original/epub/OEBPS/document_1/document_1.html#_Toc65843389> ;
    dcat:landingPage "https://www.legislation.gov.au/F2021L00312/asmade/2021-03-24/text/original/epub/OEBPS/document_1/document_1.html#_Toc65843389"^^xsd:anyURI ;
    dcat:theme legcons:Item .

F2021L00312:106 a legcons:Item,
        owl:Class,
        dcat:Resource ;
    rdfs:label "Item - I106 5 34  Establishments where eggs or egg products that are not for export etc are prepared"@en-AU ;
    dct:isPartOf F2021L00312:104 ;
    dct:isReferencedBy F2021L00312: ;
    rdfs:comment "5 34  Establishments where eggs or egg products that are not for export etc are prepared - Abrievated Graph Key: I106"@en-AU ;
    skos:definition "5 34  Establishments where eggs or egg products that are not for export etc are prepared"@en-AU ;
    skos:narrower F2021L00312:104 ;
    skos:prefLabel "Item I106"@en-AU ;
    dcat:accessURL <https://www.legislation.gov.au/F2021L00312/asmade/2021-03-24/text/original/epub/OEBPS/document_1/document_1.html#_Toc65843390> ;
    dcat:landingPage "https://www.legislation.gov.au/F2021L00312/asmade/2021-03-24/text/original/epub/OEBPS/document_1/document_1.html#_Toc65843390"^^xsd:anyURI ;
    dcat:theme legcons:Item .

F2021L00312:107 a legcons:Item,
        owl:Class,
        dcat:Resource ;
    rdfs:label "Item - I107 5 35  Integritygeneral"@en-AU ;
    dct:isPartOf F2021L00312:104 ;
    dct:isReferencedBy F2021L00312: ;
    rdfs:comment "5 35  Integritygeneral - Abrievated Graph Key: I107"@en-AU ;
    skos:definition "5 35  Integritygeneral"@en-AU ;
    skos:narrower F2021L00312:104 ;
    skos:prefLabel "Item I107"@en-AU ;
    dcat:accessURL <https://www.legislation.gov.au/F2021L00312/asmade/2021-03-24/text/original/epub/OEBPS/document_1/document_1.html#_Toc65843391> ;
    dcat:landingPage "https://www.legislation.gov.au/F2021L00312/asmade/2021-03-24/text/original/epub/OEBPS/document_1/document_1.html#_Toc65843391"^^xsd:anyURI ;
    dcat:theme legcons:Item .

F2021L00312:109 a legcons:Item,
        owl:Class,
        dcat:Resource ;
    rdfs:label "Item - I109 5 36  Information and declarations relating to transferred prescribed eggs or egg products"@en-AU ;
    dct:isPartOf F2021L00312:108 ;
    dct:isReferencedBy F2021L00312: ;
    rdfs:comment "5 36  Information and declarations relating to transferred prescribed eggs or egg products - Abrievated Graph Key: I109"@en-AU ;
    skos:definition "5 36  Information and declarations relating to transferred prescribed eggs or egg products"@en-AU ;
    skos:narrower F2021L00312:108 ;
    skos:prefLabel "Item I109"@en-AU ;
    dcat:accessURL <https://www.legislation.gov.au/F2021L00312/asmade/2021-03-24/text/original/epub/OEBPS/document_1/document_1.html#_Toc65843393> ;
    dcat:landingPage "https://www.legislation.gov.au/F2021L00312/asmade/2021-03-24/text/original/epub/OEBPS/document_1/document_1.html#_Toc65843393"^^xsd:anyURI ;
    dcat:theme legcons:Item .

F2021L00312:110 a legcons:Item,
        owl:Class,
        dcat:Resource ;
    rdfs:label "Item - I110 5 37  Information and declarations not received or inaccurate or incomplete"@en-AU ;
    dct:isPartOf F2021L00312:108 ;
    dct:isReferencedBy F2021L00312: ;
    rdfs:comment "5 37  Information and declarations not received or inaccurate or incomplete - Abrievated Graph Key: I110"@en-AU ;
    skos:definition "5 37  Information and declarations not received or inaccurate or incomplete"@en-AU ;
    skos:narrower F2021L00312:108 ;
    skos:prefLabel "Item I110"@en-AU ;
    dcat:accessURL <https://www.legislation.gov.au/F2021L00312/asmade/2021-03-24/text/original/epub/OEBPS/document_1/document_1.html#_Toc65843394> ;
    dcat:landingPage "https://www.legislation.gov.au/F2021L00312/asmade/2021-03-24/text/original/epub/OEBPS/document_1/document_1.html#_Toc65843394"^^xsd:anyURI ;
    dcat:theme legcons:Item .

F2021L00312:112 a legcons:Item,
        owl:Class,
        dcat:Resource ;
    rdfs:label "Item - I112 5 38  Management practices organisational structure resources and personnel"@en-AU ;
    dct:isPartOf F2021L00312:111 ;
    dct:isReferencedBy F2021L00312: ;
    rdfs:comment "5 38  Management practices organisational structure resources and personnel - Abrievated Graph Key: I112"@en-AU ;
    skos:definition "5 38  Management practices organisational structure resources and personnel"@en-AU ;
    skos:narrower F2021L00312:111 ;
    skos:prefLabel "Item I112"@en-AU ;
    dcat:accessURL <https://www.legislation.gov.au/F2021L00312/asmade/2021-03-24/text/original/epub/OEBPS/document_1/document_1.html#_Toc65843396> ;
    dcat:landingPage "https://www.legislation.gov.au/F2021L00312/asmade/2021-03-24/text/original/epub/OEBPS/document_1/document_1.html#_Toc65843396"^^xsd:anyURI ;
    dcat:theme legcons:Item .

F2021L00312:113 a legcons:Item,
        owl:Class,
        dcat:Resource ;
    rdfs:label "Item - I113 5 39  Verification of compliance with the Act and other matters"@en-AU ;
    dct:isPartOf F2021L00312:111 ;
    dct:isReferencedBy F2021L00312: ;
    rdfs:comment "5 39  Verification of compliance with the Act and other matters - Abrievated Graph Key: I113"@en-AU ;
    skos:definition "5 39  Verification of compliance with the Act and other matters"@en-AU ;
    skos:narrower F2021L00312:111 ;
    skos:prefLabel "Item I113"@en-AU ;
    dcat:accessURL <https://www.legislation.gov.au/F2021L00312/asmade/2021-03-24/text/original/epub/OEBPS/document_1/document_1.html#_Toc65843397> ;
    dcat:landingPage "https://www.legislation.gov.au/F2021L00312/asmade/2021-03-24/text/original/epub/OEBPS/document_1/document_1.html#_Toc65843397"^^xsd:anyURI ;
    dcat:theme legcons:Item .

F2021L00312:114 a legcons:Item,
        owl:Class,
        dcat:Resource ;
    rdfs:label "Item - I114 5 40  Action must be taken to address non compliance"@en-AU ;
    dct:isPartOf F2021L00312:111 ;
    dct:isReferencedBy F2021L00312: ;
    rdfs:comment "5 40  Action must be taken to address non compliance - Abrievated Graph Key: I114"@en-AU ;
    skos:definition "5 40  Action must be taken to address non compliance"@en-AU ;
    skos:narrower F2021L00312:111 ;
    skos:prefLabel "Item I114"@en-AU ;
    dcat:accessURL <https://www.legislation.gov.au/F2021L00312/asmade/2021-03-24/text/original/epub/OEBPS/document_1/document_1.html#_Toc65843398> ;
    dcat:landingPage "https://www.legislation.gov.au/F2021L00312/asmade/2021-03-24/text/original/epub/OEBPS/document_1/document_1.html#_Toc65843398"^^xsd:anyURI ;
    dcat:theme legcons:Item .

F2021L00312:115 a legcons:Item,
        owl:Class,
        dcat:Resource ;
    rdfs:label "Item - I115 5 41  Internal audit and management review"@en-AU ;
    dct:isPartOf F2021L00312:111 ;
    dct:isReferencedBy F2021L00312: ;
    rdfs:comment "5 41  Internal audit and management review - Abrievated Graph Key: I115"@en-AU ;
    skos:definition "5 41  Internal audit and management review"@en-AU ;
    skos:narrower F2021L00312:111 ;
    skos:prefLabel "Item I115"@en-AU ;
    dcat:accessURL <https://www.legislation.gov.au/F2021L00312/asmade/2021-03-24/text/original/epub/OEBPS/document_1/document_1.html#_Toc65843399> ;
    dcat:landingPage "https://www.legislation.gov.au/F2021L00312/asmade/2021-03-24/text/original/epub/OEBPS/document_1/document_1.html#_Toc65843399"^^xsd:anyURI ;
    dcat:theme legcons:Item .

F2021L00312:116 a legcons:Item,
        owl:Class,
        dcat:Resource ;
    rdfs:label "Item - I116 5 42  Authorised officer must be notified if prescribed eggs or egg products are not fit for human consumption or integrity cannot be ensured etc"@en-AU ;
    dct:isPartOf F2021L00312:111 ;
    dct:isReferencedBy F2021L00312: ;
    rdfs:comment "5 42  Authorised officer must be notified if prescribed eggs or egg products are not fit for human consumption or integrity cannot be ensured etc - Abrievated Graph Key: I116"@en-AU ;
    skos:definition "5 42  Authorised officer must be notified if prescribed eggs or egg products are not fit for human consumption or integrity cannot be ensured etc"@en-AU ;
    skos:narrower F2021L00312:111 ;
    skos:prefLabel "Item I116"@en-AU ;
    dcat:accessURL <https://www.legislation.gov.au/F2021L00312/asmade/2021-03-24/text/original/epub/OEBPS/document_1/document_1.html#_Toc65843400> ;
    dcat:landingPage "https://www.legislation.gov.au/F2021L00312/asmade/2021-03-24/text/original/epub/OEBPS/document_1/document_1.html#_Toc65843400"^^xsd:anyURI ;
    dcat:theme legcons:Item .

F2021L00312:118 a legcons:Item,
        owl:Class,
        dcat:Resource ;
    rdfs:label "Item - I118 5 43  Period within which application to renew approved arrangement must be made"@en-AU ;
    dct:isPartOf F2021L00312:117 ;
    dct:isReferencedBy F2021L00312: ;
    rdfs:comment "5 43  Period within which application to renew approved arrangement must be made - Abrievated Graph Key: I118"@en-AU ;
    skos:definition "5 43  Period within which application to renew approved arrangement must be made"@en-AU ;
    skos:narrower F2021L00312:117 ;
    skos:prefLabel "Item I118"@en-AU ;
    dcat:accessURL <https://www.legislation.gov.au/F2021L00312/asmade/2021-03-24/text/original/epub/OEBPS/document_1/document_1.html#_Toc65843402> ;
    dcat:landingPage "https://www.legislation.gov.au/F2021L00312/asmade/2021-03-24/text/original/epub/OEBPS/document_1/document_1.html#_Toc65843402"^^xsd:anyURI ;
    dcat:theme legcons:Item .

F2021L00312:121 a legcons:Item,
        owl:Class,
        dcat:Resource ;
    rdfs:label "Item - I121 5 44  Requirements that must be met for variation to be approved or conditions varied"@en-AU ;
    dct:isPartOf F2021L00312:120 ;
    dct:isReferencedBy F2021L00312: ;
    rdfs:comment "5 44  Requirements that must be met for variation to be approved or conditions varied - Abrievated Graph Key: I121"@en-AU ;
    skos:definition "5 44  Requirements that must be met for variation to be approved or conditions varied"@en-AU ;
    skos:narrower F2021L00312:120 ;
    skos:prefLabel "Item I121"@en-AU ;
    dcat:accessURL <https://www.legislation.gov.au/F2021L00312/asmade/2021-03-24/text/original/epub/OEBPS/document_1/document_1.html#_Toc65843405> ;
    dcat:landingPage "https://www.legislation.gov.au/F2021L00312/asmade/2021-03-24/text/original/epub/OEBPS/document_1/document_1.html#_Toc65843405"^^xsd:anyURI ;
    dcat:theme legcons:Item .

F2021L00312:122 a legcons:Item,
        owl:Class,
        dcat:Resource ;
    rdfs:label "Item - I122 5 45  Significant variations"@en-AU ;
    dct:isPartOf F2021L00312:120 ;
    dct:isReferencedBy F2021L00312: ;
    rdfs:comment "5 45  Significant variations - Abrievated Graph Key: I122"@en-AU ;
    skos:definition "5 45  Significant variations"@en-AU ;
    skos:narrower F2021L00312:120 ;
    skos:prefLabel "Item I122"@en-AU ;
    dcat:accessURL <https://www.legislation.gov.au/F2021L00312/asmade/2021-03-24/text/original/epub/OEBPS/document_1/document_1.html#_Toc65843406> ;
    dcat:landingPage "https://www.legislation.gov.au/F2021L00312/asmade/2021-03-24/text/original/epub/OEBPS/document_1/document_1.html#_Toc65843406"^^xsd:anyURI ;
    dcat:theme legcons:Item .

F2021L00312:124 a legcons:Item,
        owl:Class,
        dcat:Resource ;
    rdfs:label "Item - I124 5 46  Other reasons for requiring holder to vary approved arrangement"@en-AU ;
    dct:isPartOf F2021L00312:123 ;
    dct:isReferencedBy F2021L00312: ;
    rdfs:comment "5 46  Other reasons for requiring holder to vary approved arrangement - Abrievated Graph Key: I124"@en-AU ;
    skos:definition "5 46  Other reasons for requiring holder to vary approved arrangement"@en-AU ;
    skos:narrower F2021L00312:123 ;
    skos:prefLabel "Item I124"@en-AU ;
    dcat:accessURL <https://www.legislation.gov.au/F2021L00312/asmade/2021-03-24/text/original/epub/OEBPS/document_1/document_1.html#_Toc65843408> ;
    dcat:landingPage "https://www.legislation.gov.au/F2021L00312/asmade/2021-03-24/text/original/epub/OEBPS/document_1/document_1.html#_Toc65843408"^^xsd:anyURI ;
    dcat:theme legcons:Item .

F2021L00312:126 a legcons:Item,
        owl:Class,
        dcat:Resource ;
    rdfs:label "Item - I126 5 47  Application of this Part"@en-AU ;
    dct:isPartOf F2021L00312:125 ;
    dct:isReferencedBy F2021L00312: ;
    rdfs:comment "5 47  Application of this Part - Abrievated Graph Key: I126"@en-AU ;
    skos:definition "5 47  Application of this Part"@en-AU ;
    skos:narrower F2021L00312:125 ;
    skos:prefLabel "Item I126"@en-AU ;
    dcat:accessURL <https://www.legislation.gov.au/F2021L00312/asmade/2021-03-24/text/original/epub/OEBPS/document_1/document_1.html#_Toc65843410> ;
    dcat:landingPage "https://www.legislation.gov.au/F2021L00312/asmade/2021-03-24/text/original/epub/OEBPS/document_1/document_1.html#_Toc65843410"^^xsd:anyURI ;
    dcat:theme legcons:Item .

F2021L00312:127 a legcons:Item,
        owl:Class,
        dcat:Resource ;
    rdfs:label "Item - I127 5 48  Initial consideration period"@en-AU ;
    dct:isPartOf F2021L00312:125 ;
    dct:isReferencedBy F2021L00312: ;
    rdfs:comment "5 48  Initial consideration period - Abrievated Graph Key: I127"@en-AU ;
    skos:definition "5 48  Initial consideration period"@en-AU ;
    skos:narrower F2021L00312:125 ;
    skos:prefLabel "Item I127"@en-AU ;
    dcat:accessURL <https://www.legislation.gov.au/F2021L00312/asmade/2021-03-24/text/original/epub/OEBPS/document_1/document_1.html#_Toc65843411> ;
    dcat:landingPage "https://www.legislation.gov.au/F2021L00312/asmade/2021-03-24/text/original/epub/OEBPS/document_1/document_1.html#_Toc65843411"^^xsd:anyURI ;
    dcat:theme legcons:Item .

F2021L00312:128 a legcons:Item,
        owl:Class,
        dcat:Resource ;
    rdfs:label "Item - I128 5 49  Period within which request relating to application must be complied with"@en-AU ;
    dct:isPartOf F2021L00312:125 ;
    dct:isReferencedBy F2021L00312: ;
    rdfs:comment "5 49  Period within which request relating to application must be complied with - Abrievated Graph Key: I128"@en-AU ;
    skos:definition "5 49  Period within which request relating to application must be complied with"@en-AU ;
    skos:narrower F2021L00312:125 ;
    skos:prefLabel "Item I128"@en-AU ;
    dcat:accessURL <https://www.legislation.gov.au/F2021L00312/asmade/2021-03-24/text/original/epub/OEBPS/document_1/document_1.html#_Toc65843412> ;
    dcat:landingPage "https://www.legislation.gov.au/F2021L00312/asmade/2021-03-24/text/original/epub/OEBPS/document_1/document_1.html#_Toc65843412"^^xsd:anyURI ;
    dcat:theme legcons:Item .

F2021L00312:13 a legcons:Item,
        owl:Class,
        dcat:Resource ;
    rdfs:label "Item - I13 2 1  Eggs and egg products that are prescribed goods"@en-AU ;
    dct:isPartOf F2021L00312:12 ;
    dct:isReferencedBy F2021L00312: ;
    rdfs:comment "2 1  Eggs and egg products that are prescribed goods - Abrievated Graph Key: I13"@en-AU ;
    skos:definition "2 1  Eggs and egg products that are prescribed goods"@en-AU ;
    skos:narrower F2021L00312:12 ;
    skos:prefLabel "Item I13"@en-AU ;
    dcat:accessURL <https://www.legislation.gov.au/F2021L00312/asmade/2021-03-24/text/original/epub/OEBPS/document_1/document_1.html#_Toc65843297> ;
    dcat:landingPage "https://www.legislation.gov.au/F2021L00312/asmade/2021-03-24/text/original/epub/OEBPS/document_1/document_1.html#_Toc65843297"^^xsd:anyURI ;
    dcat:theme legcons:Item .

F2021L00312:131 a legcons:Item,
        owl:Class,
        dcat:Resource ;
    rdfs:label "Item - I131 7 1  Conditions of export permit"@en-AU ;
    dct:isPartOf F2021L00312:130 ;
    dct:isReferencedBy F2021L00312: ;
    rdfs:comment "7 1  Conditions of export permit - Abrievated Graph Key: I131"@en-AU ;
    skos:definition "7 1  Conditions of export permit"@en-AU ;
    skos:narrower F2021L00312:130 ;
    skos:prefLabel "Item I131"@en-AU ;
    dcat:accessURL <https://www.legislation.gov.au/F2021L00312/asmade/2021-03-24/text/original/epub/OEBPS/document_1/document_1.html#_Toc65843415> ;
    dcat:landingPage "https://www.legislation.gov.au/F2021L00312/asmade/2021-03-24/text/original/epub/OEBPS/document_1/document_1.html#_Toc65843415"^^xsd:anyURI ;
    dcat:theme legcons:Item .

F2021L00312:132 a legcons:Item,
        owl:Class,
        dcat:Resource ;
    rdfs:label "Item - I132 7 2  Period of effect of export permit"@en-AU ;
    dct:isPartOf F2021L00312:130 ;
    dct:isReferencedBy F2021L00312: ;
    rdfs:comment "7 2  Period of effect of export permit - Abrievated Graph Key: I132"@en-AU ;
    skos:definition "7 2  Period of effect of export permit"@en-AU ;
    skos:narrower F2021L00312:130 ;
    skos:prefLabel "Item I132"@en-AU ;
    dcat:accessURL <https://www.legislation.gov.au/F2021L00312/asmade/2021-03-24/text/original/epub/OEBPS/document_1/document_1.html#_Toc65843416> ;
    dcat:landingPage "https://www.legislation.gov.au/F2021L00312/asmade/2021-03-24/text/original/epub/OEBPS/document_1/document_1.html#_Toc65843416"^^xsd:anyURI ;
    dcat:theme legcons:Item .

F2021L00312:134 a legcons:Item,
        owl:Class,
        dcat:Resource ;
    rdfs:label "Item - I134 7 3  Period of effect of varied export permit"@en-AU ;
    dct:isPartOf F2021L00312:133 ;
    dct:isReferencedBy F2021L00312: ;
    rdfs:comment "7 3  Period of effect of varied export permit - Abrievated Graph Key: I134"@en-AU ;
    skos:definition "7 3  Period of effect of varied export permit"@en-AU ;
    skos:narrower F2021L00312:133 ;
    skos:prefLabel "Item I134"@en-AU ;
    dcat:accessURL <https://www.legislation.gov.au/F2021L00312/asmade/2021-03-24/text/original/epub/OEBPS/document_1/document_1.html#_Toc65843418> ;
    dcat:landingPage "https://www.legislation.gov.au/F2021L00312/asmade/2021-03-24/text/original/epub/OEBPS/document_1/document_1.html#_Toc65843418"^^xsd:anyURI ;
    dcat:theme legcons:Item .

F2021L00312:135 a legcons:Item,
        owl:Class,
        dcat:Resource ;
    rdfs:label "Item - I135 7 4  Circumstances in which export permit may be suspended"@en-AU ;
    dct:isPartOf F2021L00312:133 ;
    dct:isReferencedBy F2021L00312: ;
    rdfs:comment "7 4  Circumstances in which export permit may be suspended - Abrievated Graph Key: I135"@en-AU ;
    skos:definition "7 4  Circumstances in which export permit may be suspended"@en-AU ;
    skos:narrower F2021L00312:133 ;
    skos:prefLabel "Item I135"@en-AU ;
    dcat:accessURL <https://www.legislation.gov.au/F2021L00312/asmade/2021-03-24/text/original/epub/OEBPS/document_1/document_1.html#_Toc65843419> ;
    dcat:landingPage "https://www.legislation.gov.au/F2021L00312/asmade/2021-03-24/text/original/epub/OEBPS/document_1/document_1.html#_Toc65843419"^^xsd:anyURI ;
    dcat:theme legcons:Item .

F2021L00312:136 a legcons:Item,
        owl:Class,
        dcat:Resource ;
    rdfs:label "Item - I136 7 5  Other circumstances in which export permit may be revoked"@en-AU ;
    dct:isPartOf F2021L00312:133 ;
    dct:isReferencedBy F2021L00312: ;
    rdfs:comment "7 5  Other circumstances in which export permit may be revoked - Abrievated Graph Key: I136"@en-AU ;
    skos:definition "7 5  Other circumstances in which export permit may be revoked"@en-AU ;
    skos:narrower F2021L00312:133 ;
    skos:prefLabel "Item I136"@en-AU ;
    dcat:accessURL <https://www.legislation.gov.au/F2021L00312/asmade/2021-03-24/text/original/epub/OEBPS/document_1/document_1.html#_Toc65843420> ;
    dcat:landingPage "https://www.legislation.gov.au/F2021L00312/asmade/2021-03-24/text/original/epub/OEBPS/document_1/document_1.html#_Toc65843420"^^xsd:anyURI ;
    dcat:theme legcons:Item .

F2021L00312:138 a legcons:Item,
        owl:Class,
        dcat:Resource ;
    rdfs:label "Item - I138 7 6  Changes that require additional or corrected information to be given to the Secretary"@en-AU ;
    dct:isPartOf F2021L00312:137 ;
    dct:isReferencedBy F2021L00312: ;
    rdfs:comment "7 6  Changes that require additional or corrected information to be given to the Secretary - Abrievated Graph Key: I138"@en-AU ;
    skos:definition "7 6  Changes that require additional or corrected information to be given to the Secretary"@en-AU ;
    skos:narrower F2021L00312:137 ;
    skos:prefLabel "Item I138"@en-AU ;
    dcat:accessURL <https://www.legislation.gov.au/F2021L00312/asmade/2021-03-24/text/original/epub/OEBPS/document_1/document_1.html#_Toc65843422> ;
    dcat:landingPage "https://www.legislation.gov.au/F2021L00312/asmade/2021-03-24/text/original/epub/OEBPS/document_1/document_1.html#_Toc65843422"^^xsd:anyURI ;
    dcat:theme legcons:Item .

F2021L00312:139 a legcons:Item,
        owl:Class,
        dcat:Resource ;
    rdfs:label "Item - I139 7 7  Return of export permit"@en-AU ;
    dct:isPartOf F2021L00312:137 ;
    dct:isReferencedBy F2021L00312: ;
    rdfs:comment "7 7  Return of export permit - Abrievated Graph Key: I139"@en-AU ;
    skos:definition "7 7  Return of export permit"@en-AU ;
    skos:narrower F2021L00312:137 ;
    skos:prefLabel "Item I139"@en-AU ;
    dcat:accessURL <https://www.legislation.gov.au/F2021L00312/asmade/2021-03-24/text/original/epub/OEBPS/document_1/document_1.html#_Toc65843423> ;
    dcat:landingPage "https://www.legislation.gov.au/F2021L00312/asmade/2021-03-24/text/original/epub/OEBPS/document_1/document_1.html#_Toc65843423"^^xsd:anyURI ;
    dcat:theme legcons:Item .

F2021L00312:14 a legcons:Item,
        owl:Class,
        dcat:Resource ;
    rdfs:label "Item - I14 2 2  Eggs and egg products that are taken not to be prescribed goods"@en-AU ;
    dct:isPartOf F2021L00312:12 ;
    dct:isReferencedBy F2021L00312: ;
    rdfs:comment "2 2  Eggs and egg products that are taken not to be prescribed goods - Abrievated Graph Key: I14"@en-AU ;
    skos:definition "2 2  Eggs and egg products that are taken not to be prescribed goods"@en-AU ;
    skos:narrower F2021L00312:12 ;
    skos:prefLabel "Item I14"@en-AU ;
    dcat:accessURL <https://www.legislation.gov.au/F2021L00312/asmade/2021-03-24/text/original/epub/OEBPS/document_1/document_1.html#_Toc65843298> ;
    dcat:landingPage "https://www.legislation.gov.au/F2021L00312/asmade/2021-03-24/text/original/epub/OEBPS/document_1/document_1.html#_Toc65843298"^^xsd:anyURI ;
    dcat:theme legcons:Item .

F2021L00312:140 a legcons:Item,
        owl:Class,
        dcat:Resource ;
    rdfs:label "Item - I140 7 8  Notification that prescribed eggs or egg products are not to be exported"@en-AU ;
    dct:isPartOf F2021L00312:137 ;
    dct:isReferencedBy F2021L00312: ;
    rdfs:comment "7 8  Notification that prescribed eggs or egg products are not to be exported - Abrievated Graph Key: I140"@en-AU ;
    skos:definition "7 8  Notification that prescribed eggs or egg products are not to be exported"@en-AU ;
    skos:narrower F2021L00312:137 ;
    skos:prefLabel "Item I140"@en-AU ;
    dcat:accessURL <https://www.legislation.gov.au/F2021L00312/asmade/2021-03-24/text/original/epub/OEBPS/document_1/document_1.html#_Toc65843424> ;
    dcat:landingPage "https://www.legislation.gov.au/F2021L00312/asmade/2021-03-24/text/original/epub/OEBPS/document_1/document_1.html#_Toc65843424"^^xsd:anyURI ;
    dcat:theme legcons:Item .

F2021L00312:142 a legcons:Item,
        owl:Class,
        dcat:Resource ;
    rdfs:label "Item - I142 7 9  Application of this Part"@en-AU ;
    dct:isPartOf F2021L00312:141 ;
    dct:isReferencedBy F2021L00312: ;
    rdfs:comment "7 9  Application of this Part - Abrievated Graph Key: I142"@en-AU ;
    skos:definition "7 9  Application of this Part"@en-AU ;
    skos:narrower F2021L00312:141 ;
    skos:prefLabel "Item I142"@en-AU ;
    dcat:accessURL <https://www.legislation.gov.au/F2021L00312/asmade/2021-03-24/text/original/epub/OEBPS/document_1/document_1.html#_Toc65843426> ;
    dcat:landingPage "https://www.legislation.gov.au/F2021L00312/asmade/2021-03-24/text/original/epub/OEBPS/document_1/document_1.html#_Toc65843426"^^xsd:anyURI ;
    dcat:theme legcons:Item .

F2021L00312:143 a legcons:Item,
        owl:Class,
        dcat:Resource ;
    rdfs:label "Item - I143 7 10  Documents to accompany application"@en-AU ;
    dct:isPartOf F2021L00312:141 ;
    dct:isReferencedBy F2021L00312: ;
    rdfs:comment "7 10  Documents to accompany application - Abrievated Graph Key: I143"@en-AU ;
    skos:definition "7 10  Documents to accompany application"@en-AU ;
    skos:narrower F2021L00312:141 ;
    skos:prefLabel "Item I143"@en-AU ;
    dcat:accessURL <https://www.legislation.gov.au/F2021L00312/asmade/2021-03-24/text/original/epub/OEBPS/document_1/document_1.html#_Toc65843427> ;
    dcat:landingPage "https://www.legislation.gov.au/F2021L00312/asmade/2021-03-24/text/original/epub/OEBPS/document_1/document_1.html#_Toc65843427"^^xsd:anyURI ;
    dcat:theme legcons:Item .

F2021L00312:146 a legcons:Item,
        owl:Class,
        dcat:Resource ;
    rdfs:label "Item - I146 8 1  Purpose of this Part"@en-AU ;
    dct:isPartOf F2021L00312:145 ;
    dct:isReferencedBy F2021L00312: ;
    rdfs:comment "8 1  Purpose of this Part - Abrievated Graph Key: I146"@en-AU ;
    skos:definition "8 1  Purpose of this Part"@en-AU ;
    skos:narrower F2021L00312:145 ;
    skos:prefLabel "Item I146"@en-AU ;
    dcat:accessURL <https://www.legislation.gov.au/F2021L00312/asmade/2021-03-24/text/original/epub/OEBPS/document_1/document_1.html#_Toc65843430> ;
    dcat:landingPage "https://www.legislation.gov.au/F2021L00312/asmade/2021-03-24/text/original/epub/OEBPS/document_1/document_1.html#_Toc65843430"^^xsd:anyURI ;
    dcat:theme legcons:Item .

F2021L00312:147 a legcons:Item,
        owl:Class,
        dcat:Resource ;
    rdfs:label "Item - I147 8 2  General requirements for trade descriptions"@en-AU ;
    dct:isPartOf F2021L00312:145 ;
    dct:isReferencedBy F2021L00312: ;
    rdfs:comment "8 2  General requirements for trade descriptions - Abrievated Graph Key: I147"@en-AU ;
    skos:definition "8 2  General requirements for trade descriptions"@en-AU ;
    skos:narrower F2021L00312:145 ;
    skos:prefLabel "Item I147"@en-AU ;
    dcat:accessURL <https://www.legislation.gov.au/F2021L00312/asmade/2021-03-24/text/original/epub/OEBPS/document_1/document_1.html#_Toc65843431> ;
    dcat:landingPage "https://www.legislation.gov.au/F2021L00312/asmade/2021-03-24/text/original/epub/OEBPS/document_1/document_1.html#_Toc65843431"^^xsd:anyURI ;
    dcat:theme legcons:Item .

F2021L00312:148 a legcons:Item,
        owl:Class,
        dcat:Resource ;
    rdfs:label "Item - I148 8 3  Trade descriptions in language other than English"@en-AU ;
    dct:isPartOf F2021L00312:145 ;
    dct:isReferencedBy F2021L00312: ;
    rdfs:comment "8 3  Trade descriptions in language other than English - Abrievated Graph Key: I148"@en-AU ;
    skos:definition "8 3  Trade descriptions in language other than English"@en-AU ;
    skos:narrower F2021L00312:145 ;
    skos:prefLabel "Item I148"@en-AU ;
    dcat:accessURL <https://www.legislation.gov.au/F2021L00312/asmade/2021-03-24/text/original/epub/OEBPS/document_1/document_1.html#_Toc65843432> ;
    dcat:landingPage "https://www.legislation.gov.au/F2021L00312/asmade/2021-03-24/text/original/epub/OEBPS/document_1/document_1.html#_Toc65843432"^^xsd:anyURI ;
    dcat:theme legcons:Item .

F2021L00312:15 a legcons:Division,
        owl:Class,
        dcat:Resource ;
    rdfs:label "Division - D15 Division 2 Prohibited export and prescribed export conditions"@en-AU ;
    dct:isPartOf F2021L00312:11 ;
    dct:isReferencedBy F2021L00312: ;
    rdfs:comment "Division 2 Prohibited export and prescribed export conditions - Abrievated Graph Key: D15"@en-AU ;
    skos:definition "Division 2 Prohibited export and prescribed export conditions"@en-AU ;
    skos:narrower F2021L00312:11 ;
    skos:prefLabel "Division D15"@en-AU ;
    dcat:accessURL <https://www.legislation.gov.au/F2021L00312/asmade/2021-03-24/text/original/epub/OEBPS/document_1/document_1.html#_Toc65843299> ;
    dcat:landingPage "https://www.legislation.gov.au/F2021L00312/asmade/2021-03-24/text/original/epub/OEBPS/document_1/document_1.html#_Toc65843299"^^xsd:anyURI ;
    dcat:theme legcons:Division .

F2021L00312:151 a legcons:Item,
        owl:Class,
        dcat:Resource ;
    rdfs:label "Item - I151 8 4  Purpose of this Division"@en-AU ;
    dct:isPartOf F2021L00312:150 ;
    dct:isReferencedBy F2021L00312: ;
    rdfs:comment "8 4  Purpose of this Division - Abrievated Graph Key: I151"@en-AU ;
    skos:definition "8 4  Purpose of this Division"@en-AU ;
    skos:narrower F2021L00312:150 ;
    skos:prefLabel "Item I151"@en-AU ;
    dcat:accessURL <https://www.legislation.gov.au/F2021L00312/asmade/2021-03-24/text/original/epub/OEBPS/document_1/document_1.html#_Toc65843435> ;
    dcat:landingPage "https://www.legislation.gov.au/F2021L00312/asmade/2021-03-24/text/original/epub/OEBPS/document_1/document_1.html#_Toc65843435"^^xsd:anyURI ;
    dcat:theme legcons:Item .

F2021L00312:152 a legcons:Item,
        owl:Class,
        dcat:Resource ;
    rdfs:label "Item - I152 8 5  Tolerances for dimensions of official marks"@en-AU ;
    dct:isPartOf F2021L00312:150 ;
    dct:isReferencedBy F2021L00312: ;
    rdfs:comment "8 5  Tolerances for dimensions of official marks - Abrievated Graph Key: I152"@en-AU ;
    skos:definition "8 5  Tolerances for dimensions of official marks"@en-AU ;
    skos:narrower F2021L00312:150 ;
    skos:prefLabel "Item I152"@en-AU ;
    dcat:accessURL <https://www.legislation.gov.au/F2021L00312/asmade/2021-03-24/text/original/epub/OEBPS/document_1/document_1.html#_Toc65843436> ;
    dcat:landingPage "https://www.legislation.gov.au/F2021L00312/asmade/2021-03-24/text/original/epub/OEBPS/document_1/document_1.html#_Toc65843436"^^xsd:anyURI ;
    dcat:theme legcons:Item .

F2021L00312:153 a legcons:Item,
        owl:Class,
        dcat:Resource ;
    rdfs:label "Item - I153 8 6  Official markforeign country identification"@en-AU ;
    dct:isPartOf F2021L00312:150 ;
    dct:isReferencedBy F2021L00312: ;
    rdfs:comment "8 6  Official markforeign country identification - Abrievated Graph Key: I153"@en-AU ;
    skos:definition "8 6  Official markforeign country identification"@en-AU ;
    skos:narrower F2021L00312:150 ;
    skos:prefLabel "Item I153"@en-AU ;
    dcat:accessURL <https://www.legislation.gov.au/F2021L00312/asmade/2021-03-24/text/original/epub/OEBPS/document_1/document_1.html#_Toc65843437> ;
    dcat:landingPage "https://www.legislation.gov.au/F2021L00312/asmade/2021-03-24/text/original/epub/OEBPS/document_1/document_1.html#_Toc65843437"^^xsd:anyURI ;
    dcat:theme legcons:Item .

F2021L00312:154 a legcons:Item,
        owl:Class,
        dcat:Resource ;
    rdfs:label "Item - I154 8 7  Official marktamper indicative metal strap seal"@en-AU ;
    dct:isPartOf F2021L00312:150 ;
    dct:isReferencedBy F2021L00312: ;
    rdfs:comment "8 7  Official marktamper indicative metal strap seal - Abrievated Graph Key: I154"@en-AU ;
    skos:definition "8 7  Official marktamper indicative metal strap seal"@en-AU ;
    skos:narrower F2021L00312:150 ;
    skos:prefLabel "Item I154"@en-AU ;
    dcat:accessURL <https://www.legislation.gov.au/F2021L00312/asmade/2021-03-24/text/original/epub/OEBPS/document_1/document_1.html#_Toc65843438> ;
    dcat:landingPage "https://www.legislation.gov.au/F2021L00312/asmade/2021-03-24/text/original/epub/OEBPS/document_1/document_1.html#_Toc65843438"^^xsd:anyURI ;
    dcat:theme legcons:Item .

F2021L00312:155 a legcons:Item,
        owl:Class,
        dcat:Resource ;
    rdfs:label "Item - I155 8 8  Official markbolt seal"@en-AU ;
    dct:isPartOf F2021L00312:150 ;
    dct:isReferencedBy F2021L00312: ;
    rdfs:comment "8 8  Official markbolt seal - Abrievated Graph Key: I155"@en-AU ;
    skos:definition "8 8  Official markbolt seal"@en-AU ;
    skos:narrower F2021L00312:150 ;
    skos:prefLabel "Item I155"@en-AU ;
    dcat:accessURL <https://www.legislation.gov.au/F2021L00312/asmade/2021-03-24/text/original/epub/OEBPS/document_1/document_1.html#_Toc65843439> ;
    dcat:landingPage "https://www.legislation.gov.au/F2021L00312/asmade/2021-03-24/text/original/epub/OEBPS/document_1/document_1.html#_Toc65843439"^^xsd:anyURI ;
    dcat:theme legcons:Item .

F2021L00312:156 a legcons:Item,
        owl:Class,
        dcat:Resource ;
    rdfs:label "Item - I156 8 9  Official markEuropean Union"@en-AU ;
    dct:isPartOf F2021L00312:150 ;
    dct:isReferencedBy F2021L00312: ;
    rdfs:comment "8 9  Official markEuropean Union - Abrievated Graph Key: I156"@en-AU ;
    skos:definition "8 9  Official markEuropean Union"@en-AU ;
    skos:narrower F2021L00312:150 ;
    skos:prefLabel "Item I156"@en-AU ;
    dcat:accessURL <https://www.legislation.gov.au/F2021L00312/asmade/2021-03-24/text/original/epub/OEBPS/document_1/document_1.html#_Toc65843440> ;
    dcat:landingPage "https://www.legislation.gov.au/F2021L00312/asmade/2021-03-24/text/original/epub/OEBPS/document_1/document_1.html#_Toc65843440"^^xsd:anyURI ;
    dcat:theme legcons:Item .

F2021L00312:157 a legcons:Item,
        owl:Class,
        dcat:Resource ;
    rdfs:label "Item - I157 8 10  Official markcarton seal"@en-AU ;
    dct:isPartOf F2021L00312:150 ;
    dct:isReferencedBy F2021L00312: ;
    rdfs:comment "8 10  Official markcarton seal - Abrievated Graph Key: I157"@en-AU ;
    skos:definition "8 10  Official markcarton seal"@en-AU ;
    skos:narrower F2021L00312:150 ;
    skos:prefLabel "Item I157"@en-AU ;
    dcat:accessURL <https://www.legislation.gov.au/F2021L00312/asmade/2021-03-24/text/original/epub/OEBPS/document_1/document_1.html#_Toc65843441> ;
    dcat:landingPage "https://www.legislation.gov.au/F2021L00312/asmade/2021-03-24/text/original/epub/OEBPS/document_1/document_1.html#_Toc65843441"^^xsd:anyURI ;
    dcat:theme legcons:Item .

F2021L00312:158 a legcons:Item,
        owl:Class,
        dcat:Resource ;
    rdfs:label "Item - I158 8 11  Official markgoods opened for assessment and resealed"@en-AU ;
    dct:isPartOf F2021L00312:150 ;
    dct:isReferencedBy F2021L00312: ;
    rdfs:comment "8 11  Official markgoods opened for assessment and resealed - Abrievated Graph Key: I158"@en-AU ;
    skos:definition "8 11  Official markgoods opened for assessment and resealed"@en-AU ;
    skos:narrower F2021L00312:150 ;
    skos:prefLabel "Item I158"@en-AU ;
    dcat:accessURL <https://www.legislation.gov.au/F2021L00312/asmade/2021-03-24/text/original/epub/OEBPS/document_1/document_1.html#_Toc65843442> ;
    dcat:landingPage "https://www.legislation.gov.au/F2021L00312/asmade/2021-03-24/text/original/epub/OEBPS/document_1/document_1.html#_Toc65843442"^^xsd:anyURI ;
    dcat:theme legcons:Item .

F2021L00312:159 a legcons:Item,
        owl:Class,
        dcat:Resource ;
    rdfs:label "Item - I159 8 12  Official markAustralian Government"@en-AU ;
    dct:isPartOf F2021L00312:150 ;
    dct:isReferencedBy F2021L00312: ;
    rdfs:comment "8 12  Official markAustralian Government - Abrievated Graph Key: I159"@en-AU ;
    skos:definition "8 12  Official markAustralian Government"@en-AU ;
    skos:narrower F2021L00312:150 ;
    skos:prefLabel "Item I159"@en-AU ;
    dcat:accessURL <https://www.legislation.gov.au/F2021L00312/asmade/2021-03-24/text/original/epub/OEBPS/document_1/document_1.html#_Toc65843443> ;
    dcat:landingPage "https://www.legislation.gov.au/F2021L00312/asmade/2021-03-24/text/original/epub/OEBPS/document_1/document_1.html#_Toc65843443"^^xsd:anyURI ;
    dcat:theme legcons:Item .

F2021L00312:16 a legcons:Item,
        owl:Class,
        dcat:Resource ;
    rdfs:label "Item - I16 2 3  Purpose and application of this Division"@en-AU ;
    dct:isPartOf F2021L00312:11 ;
    dct:isReferencedBy F2021L00312: ;
    rdfs:comment "2 3  Purpose and application of this Division - Abrievated Graph Key: I16"@en-AU ;
    skos:definition "2 3  Purpose and application of this Division"@en-AU ;
    skos:narrower F2021L00312:11 ;
    skos:prefLabel "Item I16"@en-AU ;
    dcat:accessURL <https://www.legislation.gov.au/F2021L00312/asmade/2021-03-24/text/original/epub/OEBPS/document_1/document_1.html#_Toc65843300> ;
    dcat:landingPage "https://www.legislation.gov.au/F2021L00312/asmade/2021-03-24/text/original/epub/OEBPS/document_1/document_1.html#_Toc65843300"^^xsd:anyURI ;
    dcat:theme legcons:Item .

F2021L00312:161 a legcons:Item,
        owl:Class,
        dcat:Resource ;
    rdfs:label "Item - I161 8 13  Purpose and application of this Division"@en-AU ;
    dct:isPartOf F2021L00312:160 ;
    dct:isReferencedBy F2021L00312: ;
    rdfs:comment "8 13  Purpose and application of this Division - Abrievated Graph Key: I161"@en-AU ;
    skos:definition "8 13  Purpose and application of this Division"@en-AU ;
    skos:narrower F2021L00312:160 ;
    skos:prefLabel "Item I161"@en-AU ;
    dcat:accessURL <https://www.legislation.gov.au/F2021L00312/asmade/2021-03-24/text/original/epub/OEBPS/document_1/document_1.html#_Toc65843445> ;
    dcat:landingPage "https://www.legislation.gov.au/F2021L00312/asmade/2021-03-24/text/original/epub/OEBPS/document_1/document_1.html#_Toc65843445"^^xsd:anyURI ;
    dcat:theme legcons:Item .

F2021L00312:162 a legcons:Item,
        owl:Class,
        dcat:Resource ;
    rdfs:label "Item - I162 8 14  Interpretation"@en-AU ;
    dct:isPartOf F2021L00312:160 ;
    dct:isReferencedBy F2021L00312: ;
    rdfs:comment "8 14  Interpretation - Abrievated Graph Key: I162"@en-AU ;
    skos:definition "8 14  Interpretation"@en-AU ;
    skos:narrower F2021L00312:160 ;
    skos:prefLabel "Item I162"@en-AU ;
    dcat:accessURL <https://www.legislation.gov.au/F2021L00312/asmade/2021-03-24/text/original/epub/OEBPS/document_1/document_1.html#_Toc65843446> ;
    dcat:landingPage "https://www.legislation.gov.au/F2021L00312/asmade/2021-03-24/text/original/epub/OEBPS/document_1/document_1.html#_Toc65843446"^^xsd:anyURI ;
    dcat:theme legcons:Item .

F2021L00312:163 a legcons:Item,
        owl:Class,
        dcat:Resource ;
    rdfs:label "Item - I163 8 15  Persons who may manufacture or supply official marks for eggs or egg products"@en-AU ;
    dct:isPartOf F2021L00312:160 ;
    dct:isReferencedBy F2021L00312: ;
    rdfs:comment "8 15  Persons who may manufacture or supply official marks for eggs or egg products - Abrievated Graph Key: I163"@en-AU ;
    skos:definition "8 15  Persons who may manufacture or supply official marks for eggs or egg products"@en-AU ;
    skos:narrower F2021L00312:160 ;
    skos:prefLabel "Item I163"@en-AU ;
    dcat:accessURL <https://www.legislation.gov.au/F2021L00312/asmade/2021-03-24/text/original/epub/OEBPS/document_1/document_1.html#_Toc65843447> ;
    dcat:landingPage "https://www.legislation.gov.au/F2021L00312/asmade/2021-03-24/text/original/epub/OEBPS/document_1/document_1.html#_Toc65843447"^^xsd:anyURI ;
    dcat:theme legcons:Item .

F2021L00312:164 a legcons:Item,
        owl:Class,
        dcat:Resource ;
    rdfs:label "Item - I164 8 16  Persons who may possess official marks that have not been applied to eggs or egg products"@en-AU ;
    dct:isPartOf F2021L00312:160 ;
    dct:isReferencedBy F2021L00312: ;
    rdfs:comment "8 16  Persons who may possess official marks that have not been applied to eggs or egg products - Abrievated Graph Key: I164"@en-AU ;
    skos:definition "8 16  Persons who may possess official marks that have not been applied to eggs or egg products"@en-AU ;
    skos:narrower F2021L00312:160 ;
    skos:prefLabel "Item I164"@en-AU ;
    dcat:accessURL <https://www.legislation.gov.au/F2021L00312/asmade/2021-03-24/text/original/epub/OEBPS/document_1/document_1.html#_Toc65843448> ;
    dcat:landingPage "https://www.legislation.gov.au/F2021L00312/asmade/2021-03-24/text/original/epub/OEBPS/document_1/document_1.html#_Toc65843448"^^xsd:anyURI ;
    dcat:theme legcons:Item .

F2021L00312:165 a legcons:Item,
        owl:Class,
        dcat:Resource ;
    rdfs:label "Item - I165 8 17  Persons who may apply official marks to eggs or egg products etc"@en-AU ;
    dct:isPartOf F2021L00312:160 ;
    dct:isReferencedBy F2021L00312: ;
    rdfs:comment "8 17  Persons who may apply official marks to eggs or egg products etc - Abrievated Graph Key: I165"@en-AU ;
    skos:definition "8 17  Persons who may apply official marks to eggs or egg products etc"@en-AU ;
    skos:narrower F2021L00312:160 ;
    skos:prefLabel "Item I165"@en-AU ;
    dcat:accessURL <https://www.legislation.gov.au/F2021L00312/asmade/2021-03-24/text/original/epub/OEBPS/document_1/document_1.html#_Toc65843449> ;
    dcat:landingPage "https://www.legislation.gov.au/F2021L00312/asmade/2021-03-24/text/original/epub/OEBPS/document_1/document_1.html#_Toc65843449"^^xsd:anyURI ;
    dcat:theme legcons:Item .

F2021L00312:166 a legcons:Item,
        owl:Class,
        dcat:Resource ;
    rdfs:label "Item - I166 8 18  Circumstances in which official mark must not be applied to eggs or egg products"@en-AU ;
    dct:isPartOf F2021L00312:160 ;
    dct:isReferencedBy F2021L00312: ;
    rdfs:comment "8 18  Circumstances in which official mark must not be applied to eggs or egg products - Abrievated Graph Key: I166"@en-AU ;
    skos:definition "8 18  Circumstances in which official mark must not be applied to eggs or egg products"@en-AU ;
    skos:narrower F2021L00312:160 ;
    skos:prefLabel "Item I166"@en-AU ;
    dcat:accessURL <https://www.legislation.gov.au/F2021L00312/asmade/2021-03-24/text/original/epub/OEBPS/document_1/document_1.html#_Toc65843450> ;
    dcat:landingPage "https://www.legislation.gov.au/F2021L00312/asmade/2021-03-24/text/original/epub/OEBPS/document_1/document_1.html#_Toc65843450"^^xsd:anyURI ;
    dcat:theme legcons:Item .

F2021L00312:167 a legcons:Item,
        owl:Class,
        dcat:Resource ;
    rdfs:label "Item - I167 8 19  Alteration of and interference with official marks"@en-AU ;
    dct:isPartOf F2021L00312:160 ;
    dct:isReferencedBy F2021L00312: ;
    rdfs:comment "8 19  Alteration of and interference with official marks - Abrievated Graph Key: I167"@en-AU ;
    skos:definition "8 19  Alteration of and interference with official marks"@en-AU ;
    skos:narrower F2021L00312:160 ;
    skos:prefLabel "Item I167"@en-AU ;
    dcat:accessURL <https://www.legislation.gov.au/F2021L00312/asmade/2021-03-24/text/original/epub/OEBPS/document_1/document_1.html#_Toc65843451> ;
    dcat:landingPage "https://www.legislation.gov.au/F2021L00312/asmade/2021-03-24/text/original/epub/OEBPS/document_1/document_1.html#_Toc65843451"^^xsd:anyURI ;
    dcat:theme legcons:Item .

F2021L00312:168 a legcons:Item,
        owl:Class,
        dcat:Resource ;
    rdfs:label "Item - I168 8 20  Official marks must be legible and securely attached"@en-AU ;
    dct:isPartOf F2021L00312:160 ;
    dct:isReferencedBy F2021L00312: ;
    rdfs:comment "8 20  Official marks must be legible and securely attached - Abrievated Graph Key: I168"@en-AU ;
    skos:definition "8 20  Official marks must be legible and securely attached"@en-AU ;
    skos:narrower F2021L00312:160 ;
    skos:prefLabel "Item I168"@en-AU ;
    dcat:accessURL <https://www.legislation.gov.au/F2021L00312/asmade/2021-03-24/text/original/epub/OEBPS/document_1/document_1.html#_Toc65843452> ;
    dcat:landingPage "https://www.legislation.gov.au/F2021L00312/asmade/2021-03-24/text/original/epub/OEBPS/document_1/document_1.html#_Toc65843452"^^xsd:anyURI ;
    dcat:theme legcons:Item .

F2021L00312:169 a legcons:Item,
        owl:Class,
        dcat:Resource ;
    rdfs:label "Item - I169 8 21  Security of official marks"@en-AU ;
    dct:isPartOf F2021L00312:160 ;
    dct:isReferencedBy F2021L00312: ;
    rdfs:comment "8 21  Security of official marks - Abrievated Graph Key: I169"@en-AU ;
    skos:definition "8 21  Security of official marks"@en-AU ;
    skos:narrower F2021L00312:160 ;
    skos:prefLabel "Item I169"@en-AU ;
    dcat:accessURL <https://www.legislation.gov.au/F2021L00312/asmade/2021-03-24/text/original/epub/OEBPS/document_1/document_1.html#_Toc65843453> ;
    dcat:landingPage "https://www.legislation.gov.au/F2021L00312/asmade/2021-03-24/text/original/epub/OEBPS/document_1/document_1.html#_Toc65843453"^^xsd:anyURI ;
    dcat:theme legcons:Item .

F2021L00312:17 a legcons:Item,
        owl:Class,
        dcat:Resource ;
    rdfs:label "Item - I17 2 4  Export of prescribed eggs or egg products is prohibited unless prescribed conditions are complied with"@en-AU ;
    dct:isPartOf F2021L00312:11 ;
    dct:isReferencedBy F2021L00312: ;
    rdfs:comment "2 4  Export of prescribed eggs or egg products is prohibited unless prescribed conditions are complied with - Abrievated Graph Key: I17"@en-AU ;
    skos:definition "2 4  Export of prescribed eggs or egg products is prohibited unless prescribed conditions are complied with"@en-AU ;
    skos:narrower F2021L00312:11 ;
    skos:prefLabel "Item I17"@en-AU ;
    dcat:accessURL <https://www.legislation.gov.au/F2021L00312/asmade/2021-03-24/text/original/epub/OEBPS/document_1/document_1.html#_Toc65843301> ;
    dcat:landingPage "https://www.legislation.gov.au/F2021L00312/asmade/2021-03-24/text/original/epub/OEBPS/document_1/document_1.html#_Toc65843301"^^xsd:anyURI ;
    dcat:theme legcons:Item .

F2021L00312:170 a legcons:Item,
        owl:Class,
        dcat:Resource ;
    rdfs:label "Item - I170 8 22  Removal or defacement of official marks"@en-AU ;
    dct:isPartOf F2021L00312:160 ;
    dct:isReferencedBy F2021L00312: ;
    rdfs:comment "8 22  Removal or defacement of official marks - Abrievated Graph Key: I170"@en-AU ;
    skos:definition "8 22  Removal or defacement of official marks"@en-AU ;
    skos:narrower F2021L00312:160 ;
    skos:prefLabel "Item I170"@en-AU ;
    dcat:accessURL <https://www.legislation.gov.au/F2021L00312/asmade/2021-03-24/text/original/epub/OEBPS/document_1/document_1.html#_Toc65843454> ;
    dcat:landingPage "https://www.legislation.gov.au/F2021L00312/asmade/2021-03-24/text/original/epub/OEBPS/document_1/document_1.html#_Toc65843454"^^xsd:anyURI ;
    dcat:theme legcons:Item .

F2021L00312:171 a legcons:Item,
        owl:Class,
        dcat:Resource ;
    rdfs:label "Item - I171 8 23  Records of official marks manufactured or supplied"@en-AU ;
    dct:isPartOf F2021L00312:160 ;
    dct:isReferencedBy F2021L00312: ;
    rdfs:comment "8 23  Records of official marks manufactured or supplied - Abrievated Graph Key: I171"@en-AU ;
    skos:definition "8 23  Records of official marks manufactured or supplied"@en-AU ;
    skos:narrower F2021L00312:160 ;
    skos:prefLabel "Item I171"@en-AU ;
    dcat:accessURL <https://www.legislation.gov.au/F2021L00312/asmade/2021-03-24/text/original/epub/OEBPS/document_1/document_1.html#_Toc65843455> ;
    dcat:landingPage "https://www.legislation.gov.au/F2021L00312/asmade/2021-03-24/text/original/epub/OEBPS/document_1/document_1.html#_Toc65843455"^^xsd:anyURI ;
    dcat:theme legcons:Item .

F2021L00312:172 a legcons:Item,
        owl:Class,
        dcat:Resource ;
    rdfs:label "Item - I172 8 24  Records of official marks received applied removed defaced destroyed or returned"@en-AU ;
    dct:isPartOf F2021L00312:160 ;
    dct:isReferencedBy F2021L00312: ;
    rdfs:comment "8 24  Records of official marks received applied removed defaced destroyed or returned - Abrievated Graph Key: I172"@en-AU ;
    skos:definition "8 24  Records of official marks received applied removed defaced destroyed or returned"@en-AU ;
    skos:narrower F2021L00312:160 ;
    skos:prefLabel "Item I172"@en-AU ;
    dcat:accessURL <https://www.legislation.gov.au/F2021L00312/asmade/2021-03-24/text/original/epub/OEBPS/document_1/document_1.html#_Toc65843456> ;
    dcat:landingPage "https://www.legislation.gov.au/F2021L00312/asmade/2021-03-24/text/original/epub/OEBPS/document_1/document_1.html#_Toc65843456"^^xsd:anyURI ;
    dcat:theme legcons:Item .

F2021L00312:174 a legcons:Item,
        owl:Class,
        dcat:Resource ;
    rdfs:label "Item - I174 8 25  Purpose of this Division"@en-AU ;
    dct:isPartOf F2021L00312:173 ;
    dct:isReferencedBy F2021L00312: ;
    rdfs:comment "8 25  Purpose of this Division - Abrievated Graph Key: I174"@en-AU ;
    skos:definition "8 25  Purpose of this Division"@en-AU ;
    skos:narrower F2021L00312:173 ;
    skos:prefLabel "Item I174"@en-AU ;
    dcat:accessURL <https://www.legislation.gov.au/F2021L00312/asmade/2021-03-24/text/original/epub/OEBPS/document_1/document_1.html#_Toc65843458> ;
    dcat:landingPage "https://www.legislation.gov.au/F2021L00312/asmade/2021-03-24/text/original/epub/OEBPS/document_1/document_1.html#_Toc65843458"^^xsd:anyURI ;
    dcat:theme legcons:Item .

F2021L00312:175 a legcons:Item,
        owl:Class,
        dcat:Resource ;
    rdfs:label "Item - I175 8 26  Circumstances in which a mark resembles an official mark"@en-AU ;
    dct:isPartOf F2021L00312:173 ;
    dct:isReferencedBy F2021L00312: ;
    rdfs:comment "8 26  Circumstances in which a mark resembles an official mark - Abrievated Graph Key: I175"@en-AU ;
    skos:definition "8 26  Circumstances in which a mark resembles an official mark"@en-AU ;
    skos:narrower F2021L00312:173 ;
    skos:prefLabel "Item I175"@en-AU ;
    dcat:accessURL <https://www.legislation.gov.au/F2021L00312/asmade/2021-03-24/text/original/epub/OEBPS/document_1/document_1.html#_Toc65843459> ;
    dcat:landingPage "https://www.legislation.gov.au/F2021L00312/asmade/2021-03-24/text/original/epub/OEBPS/document_1/document_1.html#_Toc65843459"^^xsd:anyURI ;
    dcat:theme legcons:Item .

F2021L00312:176 a legcons:Item,
        owl:Class,
        dcat:Resource ;
    rdfs:label "Item - I176 8 27  Persons who may apply a resemblance"@en-AU ;
    dct:isPartOf F2021L00312:173 ;
    dct:isReferencedBy F2021L00312: ;
    rdfs:comment "8 27  Persons who may apply a resemblance - Abrievated Graph Key: I176"@en-AU ;
    skos:definition "8 27  Persons who may apply a resemblance"@en-AU ;
    skos:narrower F2021L00312:173 ;
    skos:prefLabel "Item I176"@en-AU ;
    dcat:accessURL <https://www.legislation.gov.au/F2021L00312/asmade/2021-03-24/text/original/epub/OEBPS/document_1/document_1.html#_Toc65843460> ;
    dcat:landingPage "https://www.legislation.gov.au/F2021L00312/asmade/2021-03-24/text/original/epub/OEBPS/document_1/document_1.html#_Toc65843460"^^xsd:anyURI ;
    dcat:theme legcons:Item .

F2021L00312:178 a legcons:Item,
        owl:Class,
        dcat:Resource ;
    rdfs:label "Item - I178 8 28  Purpose of this Division"@en-AU ;
    dct:isPartOf F2021L00312:177 ;
    dct:isReferencedBy F2021L00312: ;
    rdfs:comment "8 28  Purpose of this Division - Abrievated Graph Key: I178"@en-AU ;
    skos:definition "8 28  Purpose of this Division"@en-AU ;
    skos:narrower F2021L00312:177 ;
    skos:prefLabel "Item I178"@en-AU ;
    dcat:accessURL <https://www.legislation.gov.au/F2021L00312/asmade/2021-03-24/text/original/epub/OEBPS/document_1/document_1.html#_Toc65843462> ;
    dcat:landingPage "https://www.legislation.gov.au/F2021L00312/asmade/2021-03-24/text/original/epub/OEBPS/document_1/document_1.html#_Toc65843462"^^xsd:anyURI ;
    dcat:theme legcons:Item .

F2021L00312:179 a legcons:Item,
        owl:Class,
        dcat:Resource ;
    rdfs:label "Item - I179 8 29  Persons who may manufacture supply or possess official marking devices"@en-AU ;
    dct:isPartOf F2021L00312:177 ;
    dct:isReferencedBy F2021L00312: ;
    rdfs:comment "8 29  Persons who may manufacture supply or possess official marking devices - Abrievated Graph Key: I179"@en-AU ;
    skos:definition "8 29  Persons who may manufacture supply or possess official marking devices"@en-AU ;
    skos:narrower F2021L00312:177 ;
    skos:prefLabel "Item I179"@en-AU ;
    dcat:accessURL <https://www.legislation.gov.au/F2021L00312/asmade/2021-03-24/text/original/epub/OEBPS/document_1/document_1.html#_Toc65843463> ;
    dcat:landingPage "https://www.legislation.gov.au/F2021L00312/asmade/2021-03-24/text/original/epub/OEBPS/document_1/document_1.html#_Toc65843463"^^xsd:anyURI ;
    dcat:theme legcons:Item .

F2021L00312:18 a legcons:Part,
        owl:Class,
        dcat:Resource ;
    rdfs:label "Part - P18 Part 2 Exemptions"@en-AU ;
    dct:isPartOf F2021L00312:10 ;
    dct:isReferencedBy F2021L00312: ;
    rdfs:comment "Part 2 Exemptions - Abrievated Graph Key: P18"@en-AU ;
    skos:definition "Part 2 Exemptions"@en-AU ;
    skos:narrower F2021L00312:10 ;
    skos:prefLabel "Part P18"@en-AU ;
    dcat:accessURL <https://www.legislation.gov.au/F2021L00312/asmade/2021-03-24/text/original/epub/OEBPS/document_1/document_1.html#_Toc65843302> ;
    dcat:landingPage "https://www.legislation.gov.au/F2021L00312/asmade/2021-03-24/text/original/epub/OEBPS/document_1/document_1.html#_Toc65843302"^^xsd:anyURI ;
    dcat:theme legcons:Part .

F2021L00312:180 a legcons:Item,
        owl:Class,
        dcat:Resource ;
    rdfs:label "Item - I180 8 30  Security of official marking devices"@en-AU ;
    dct:isPartOf F2021L00312:177 ;
    dct:isReferencedBy F2021L00312: ;
    rdfs:comment "8 30  Security of official marking devices - Abrievated Graph Key: I180"@en-AU ;
    skos:definition "8 30  Security of official marking devices"@en-AU ;
    skos:narrower F2021L00312:177 ;
    skos:prefLabel "Item I180"@en-AU ;
    dcat:accessURL <https://www.legislation.gov.au/F2021L00312/asmade/2021-03-24/text/original/epub/OEBPS/document_1/document_1.html#_Toc65843464> ;
    dcat:landingPage "https://www.legislation.gov.au/F2021L00312/asmade/2021-03-24/text/original/epub/OEBPS/document_1/document_1.html#_Toc65843464"^^xsd:anyURI ;
    dcat:theme legcons:Item .

F2021L00312:181 a legcons:Item,
        owl:Class,
        dcat:Resource ;
    rdfs:label "Item - I181 8 31  Damaged etc official marking devices"@en-AU ;
    dct:isPartOf F2021L00312:177 ;
    dct:isReferencedBy F2021L00312: ;
    rdfs:comment "8 31  Damaged etc official marking devices - Abrievated Graph Key: I181"@en-AU ;
    skos:definition "8 31  Damaged etc official marking devices"@en-AU ;
    skos:narrower F2021L00312:177 ;
    skos:prefLabel "Item I181"@en-AU ;
    dcat:accessURL <https://www.legislation.gov.au/F2021L00312/asmade/2021-03-24/text/original/epub/OEBPS/document_1/document_1.html#_Toc65843465> ;
    dcat:landingPage "https://www.legislation.gov.au/F2021L00312/asmade/2021-03-24/text/original/epub/OEBPS/document_1/document_1.html#_Toc65843465"^^xsd:anyURI ;
    dcat:theme legcons:Item .

F2021L00312:182 a legcons:Item,
        owl:Class,
        dcat:Resource ;
    rdfs:label "Item - I182 8 32  Records of official marking devices manufactured or supplied"@en-AU ;
    dct:isPartOf F2021L00312:177 ;
    dct:isReferencedBy F2021L00312: ;
    rdfs:comment "8 32  Records of official marking devices manufactured or supplied - Abrievated Graph Key: I182"@en-AU ;
    skos:definition "8 32  Records of official marking devices manufactured or supplied"@en-AU ;
    skos:narrower F2021L00312:177 ;
    skos:prefLabel "Item I182"@en-AU ;
    dcat:accessURL <https://www.legislation.gov.au/F2021L00312/asmade/2021-03-24/text/original/epub/OEBPS/document_1/document_1.html#_Toc65843466> ;
    dcat:landingPage "https://www.legislation.gov.au/F2021L00312/asmade/2021-03-24/text/original/epub/OEBPS/document_1/document_1.html#_Toc65843466"^^xsd:anyURI ;
    dcat:theme legcons:Item .

F2021L00312:183 a legcons:Item,
        owl:Class,
        dcat:Resource ;
    rdfs:label "Item - I183 8 33  Records of official marking devices received used damaged destroyed or returned"@en-AU ;
    dct:isPartOf F2021L00312:177 ;
    dct:isReferencedBy F2021L00312: ;
    rdfs:comment "8 33  Records of official marking devices received used damaged destroyed or returned - Abrievated Graph Key: I183"@en-AU ;
    skos:definition "8 33  Records of official marking devices received used damaged destroyed or returned"@en-AU ;
    skos:narrower F2021L00312:177 ;
    skos:prefLabel "Item I183"@en-AU ;
    dcat:accessURL <https://www.legislation.gov.au/F2021L00312/asmade/2021-03-24/text/original/epub/OEBPS/document_1/document_1.html#_Toc65843467> ;
    dcat:landingPage "https://www.legislation.gov.au/F2021L00312/asmade/2021-03-24/text/original/epub/OEBPS/document_1/document_1.html#_Toc65843467"^^xsd:anyURI ;
    dcat:theme legcons:Item .

F2021L00312:187 a legcons:Item,
        owl:Class,
        dcat:Resource ;
    rdfs:label "Item - I187 9 1  References to audit in this Part"@en-AU ;
    dct:isPartOf F2021L00312:186 ;
    dct:isReferencedBy F2021L00312: ;
    rdfs:comment "9 1  References to audit in this Part - Abrievated Graph Key: I187"@en-AU ;
    skos:definition "9 1  References to audit in this Part"@en-AU ;
    skos:narrower F2021L00312:186 ;
    skos:prefLabel "Item I187"@en-AU ;
    dcat:accessURL <https://www.legislation.gov.au/F2021L00312/asmade/2021-03-24/text/original/epub/OEBPS/document_1/document_1.html#_Toc65843471> ;
    dcat:landingPage "https://www.legislation.gov.au/F2021L00312/asmade/2021-03-24/text/original/epub/OEBPS/document_1/document_1.html#_Toc65843471"^^xsd:anyURI ;
    dcat:theme legcons:Item .

F2021L00312:188 a legcons:Item,
        owl:Class,
        dcat:Resource ;
    rdfs:label "Item - I188 9 2  Audits of export operations"@en-AU ;
    dct:isPartOf F2021L00312:186 ;
    dct:isReferencedBy F2021L00312: ;
    rdfs:comment "9 2  Audits of export operations - Abrievated Graph Key: I188"@en-AU ;
    skos:definition "9 2  Audits of export operations"@en-AU ;
    skos:narrower F2021L00312:186 ;
    skos:prefLabel "Item I188"@en-AU ;
    dcat:accessURL <https://www.legislation.gov.au/F2021L00312/asmade/2021-03-24/text/original/epub/OEBPS/document_1/document_1.html#_Toc65843472> ;
    dcat:landingPage "https://www.legislation.gov.au/F2021L00312/asmade/2021-03-24/text/original/epub/OEBPS/document_1/document_1.html#_Toc65843472"^^xsd:anyURI ;
    dcat:theme legcons:Item .

F2021L00312:19 a legcons:Item,
        owl:Class,
        dcat:Resource ;
    rdfs:label "Item - I19 2 5  Application of this Part"@en-AU ;
    dct:isPartOf F2021L00312:10 ;
    dct:isReferencedBy F2021L00312: ;
    rdfs:comment "2 5  Application of this Part - Abrievated Graph Key: I19"@en-AU ;
    skos:definition "2 5  Application of this Part"@en-AU ;
    skos:narrower F2021L00312:10 ;
    skos:prefLabel "Item I19"@en-AU ;
    dcat:accessURL <https://www.legislation.gov.au/F2021L00312/asmade/2021-03-24/text/original/epub/OEBPS/document_1/document_1.html#_Toc65843303> ;
    dcat:landingPage "https://www.legislation.gov.au/F2021L00312/asmade/2021-03-24/text/original/epub/OEBPS/document_1/document_1.html#_Toc65843303"^^xsd:anyURI ;
    dcat:theme legcons:Item .

F2021L00312:190 a legcons:Item,
        owl:Class,
        dcat:Resource ;
    rdfs:label "Item - I190 9 3  Purpose of this Division"@en-AU ;
    dct:isPartOf F2021L00312:189 ;
    dct:isReferencedBy F2021L00312: ;
    rdfs:comment "9 3  Purpose of this Division - Abrievated Graph Key: I190"@en-AU ;
    skos:definition "9 3  Purpose of this Division"@en-AU ;
    skos:narrower F2021L00312:189 ;
    skos:prefLabel "Item I190"@en-AU ;
    dcat:accessURL <https://www.legislation.gov.au/F2021L00312/asmade/2021-03-24/text/original/epub/OEBPS/document_1/document_1.html#_Toc65843474> ;
    dcat:landingPage "https://www.legislation.gov.au/F2021L00312/asmade/2021-03-24/text/original/epub/OEBPS/document_1/document_1.html#_Toc65843474"^^xsd:anyURI ;
    dcat:theme legcons:Item .

F2021L00312:191 a legcons:Item,
        owl:Class,
        dcat:Resource ;
    rdfs:label "Item - I191 9 4  Manner in which audit must be conducted"@en-AU ;
    dct:isPartOf F2021L00312:189 ;
    dct:isReferencedBy F2021L00312: ;
    rdfs:comment "9 4  Manner in which audit must be conducted - Abrievated Graph Key: I191"@en-AU ;
    skos:definition "9 4  Manner in which audit must be conducted"@en-AU ;
    skos:narrower F2021L00312:189 ;
    skos:prefLabel "Item I191"@en-AU ;
    dcat:accessURL <https://www.legislation.gov.au/F2021L00312/asmade/2021-03-24/text/original/epub/OEBPS/document_1/document_1.html#_Toc65843475> ;
    dcat:landingPage "https://www.legislation.gov.au/F2021L00312/asmade/2021-03-24/text/original/epub/OEBPS/document_1/document_1.html#_Toc65843475"^^xsd:anyURI ;
    dcat:theme legcons:Item .

F2021L00312:192 a legcons:Item,
        owl:Class,
        dcat:Resource ;
    rdfs:label "Item - I192 9 5  Notice of non compliance with requirements"@en-AU ;
    dct:isPartOf F2021L00312:189 ;
    dct:isReferencedBy F2021L00312: ;
    rdfs:comment "9 5  Notice of non compliance with requirements - Abrievated Graph Key: I192"@en-AU ;
    skos:definition "9 5  Notice of non compliance with requirements"@en-AU ;
    skos:narrower F2021L00312:189 ;
    skos:prefLabel "Item I192"@en-AU ;
    dcat:accessURL <https://www.legislation.gov.au/F2021L00312/asmade/2021-03-24/text/original/epub/OEBPS/document_1/document_1.html#_Toc65843476> ;
    dcat:landingPage "https://www.legislation.gov.au/F2021L00312/asmade/2021-03-24/text/original/epub/OEBPS/document_1/document_1.html#_Toc65843476"^^xsd:anyURI ;
    dcat:theme legcons:Item .

F2021L00312:193 a legcons:Item,
        owl:Class,
        dcat:Resource ;
    rdfs:label "Item - I193 9 6  Audit reports"@en-AU ;
    dct:isPartOf F2021L00312:189 ;
    dct:isReferencedBy F2021L00312: ;
    rdfs:comment "9 6  Audit reports - Abrievated Graph Key: I193"@en-AU ;
    skos:definition "9 6  Audit reports"@en-AU ;
    skos:narrower F2021L00312:189 ;
    skos:prefLabel "Item I193"@en-AU ;
    dcat:accessURL <https://www.legislation.gov.au/F2021L00312/asmade/2021-03-24/text/original/epub/OEBPS/document_1/document_1.html#_Toc65843477> ;
    dcat:landingPage "https://www.legislation.gov.au/F2021L00312/asmade/2021-03-24/text/original/epub/OEBPS/document_1/document_1.html#_Toc65843477"^^xsd:anyURI ;
    dcat:theme legcons:Item .

F2021L00312:195 a legcons:Item,
        owl:Class,
        dcat:Resource ;
    rdfs:label "Item - I195 9 7  Purpose of this Division"@en-AU ;
    dct:isPartOf F2021L00312:194 ;
    dct:isReferencedBy F2021L00312: ;
    rdfs:comment "9 7  Purpose of this Division - Abrievated Graph Key: I195"@en-AU ;
    skos:definition "9 7  Purpose of this Division"@en-AU ;
    skos:narrower F2021L00312:194 ;
    skos:prefLabel "Item I195"@en-AU ;
    dcat:accessURL <https://www.legislation.gov.au/F2021L00312/asmade/2021-03-24/text/original/epub/OEBPS/document_1/document_1.html#_Toc65843479> ;
    dcat:landingPage "https://www.legislation.gov.au/F2021L00312/asmade/2021-03-24/text/original/epub/OEBPS/document_1/document_1.html#_Toc65843479"^^xsd:anyURI ;
    dcat:theme legcons:Item .

F2021L00312:196 a legcons:Item,
        owl:Class,
        dcat:Resource ;
    rdfs:label "Item - I196 9 8  Application for approval"@en-AU ;
    dct:isPartOf F2021L00312:194 ;
    dct:isReferencedBy F2021L00312: ;
    rdfs:comment "9 8  Application for approval - Abrievated Graph Key: I196"@en-AU ;
    skos:definition "9 8  Application for approval"@en-AU ;
    skos:narrower F2021L00312:194 ;
    skos:prefLabel "Item I196"@en-AU ;
    dcat:accessURL <https://www.legislation.gov.au/F2021L00312/asmade/2021-03-24/text/original/epub/OEBPS/document_1/document_1.html#_Toc65843480> ;
    dcat:landingPage "https://www.legislation.gov.au/F2021L00312/asmade/2021-03-24/text/original/epub/OEBPS/document_1/document_1.html#_Toc65843480"^^xsd:anyURI ;
    dcat:theme legcons:Item .

F2021L00312:197 a legcons:Item,
        owl:Class,
        dcat:Resource ;
    rdfs:label "Item - I197 9 9  Secretary must decide whether to approve applicant to conduct audits"@en-AU ;
    dct:isPartOf F2021L00312:194 ;
    dct:isReferencedBy F2021L00312: ;
    rdfs:comment "9 9  Secretary must decide whether to approve applicant to conduct audits - Abrievated Graph Key: I197"@en-AU ;
    skos:definition "9 9  Secretary must decide whether to approve applicant to conduct audits"@en-AU ;
    skos:narrower F2021L00312:194 ;
    skos:prefLabel "Item I197"@en-AU ;
    dcat:accessURL <https://www.legislation.gov.au/F2021L00312/asmade/2021-03-24/text/original/epub/OEBPS/document_1/document_1.html#_Toc65843481> ;
    dcat:landingPage "https://www.legislation.gov.au/F2021L00312/asmade/2021-03-24/text/original/epub/OEBPS/document_1/document_1.html#_Toc65843481"^^xsd:anyURI ;
    dcat:theme legcons:Item .

F2021L00312:198 a legcons:Item,
        owl:Class,
        dcat:Resource ;
    rdfs:label "Item - I198 9 10  Dealing with applications"@en-AU ;
    dct:isPartOf F2021L00312:194 ;
    dct:isReferencedBy F2021L00312: ;
    rdfs:comment "9 10  Dealing with applications - Abrievated Graph Key: I198"@en-AU ;
    skos:definition "9 10  Dealing with applications"@en-AU ;
    skos:narrower F2021L00312:194 ;
    skos:prefLabel "Item I198"@en-AU ;
    dcat:accessURL <https://www.legislation.gov.au/F2021L00312/asmade/2021-03-24/text/original/epub/OEBPS/document_1/document_1.html#_Toc65843482> ;
    dcat:landingPage "https://www.legislation.gov.au/F2021L00312/asmade/2021-03-24/text/original/epub/OEBPS/document_1/document_1.html#_Toc65843482"^^xsd:anyURI ;
    dcat:theme legcons:Item .

F2021L00312:199 a legcons:Item,
        owl:Class,
        dcat:Resource ;
    rdfs:label "Item - I199 9 11  Conditions of approval"@en-AU ;
    dct:isPartOf F2021L00312:194 ;
    dct:isReferencedBy F2021L00312: ;
    rdfs:comment "9 11  Conditions of approval - Abrievated Graph Key: I199"@en-AU ;
    skos:definition "9 11  Conditions of approval"@en-AU ;
    skos:narrower F2021L00312:194 ;
    skos:prefLabel "Item I199"@en-AU ;
    dcat:accessURL <https://www.legislation.gov.au/F2021L00312/asmade/2021-03-24/text/original/epub/OEBPS/document_1/document_1.html#_Toc65843483> ;
    dcat:landingPage "https://www.legislation.gov.au/F2021L00312/asmade/2021-03-24/text/original/epub/OEBPS/document_1/document_1.html#_Toc65843483"^^xsd:anyURI ;
    dcat:theme legcons:Item .

F2021L00312:2 a legcons:Part,
        owl:Class,
        dcat:Resource ;
    rdfs:label "Part - P2 Part 1 Preliminary"@en-AU ;
    dct:isPartOf F2021L00312:1 ;
    dct:isReferencedBy F2021L00312: ;
    rdfs:comment "Part 1 Preliminary - Abrievated Graph Key: P2"@en-AU ;
    skos:definition "Part 1 Preliminary"@en-AU ;
    skos:narrower F2021L00312:1 ;
    skos:prefLabel "Part P2"@en-AU ;
    dcat:accessURL <https://www.legislation.gov.au/F2021L00312/asmade/2021-03-24/text/original/epub/OEBPS/document_1/document_1.html#_Toc65843286> ;
    dcat:landingPage "https://www.legislation.gov.au/F2021L00312/asmade/2021-03-24/text/original/epub/OEBPS/document_1/document_1.html#_Toc65843286"^^xsd:anyURI ;
    dcat:theme legcons:Part .

F2021L00312:20 a legcons:Item,
        owl:Class,
        dcat:Resource ;
    rdfs:label "Item - I20 2 6  Prescribed circumstancetesting the market"@en-AU ;
    dct:isPartOf F2021L00312:10 ;
    dct:isReferencedBy F2021L00312: ;
    rdfs:comment "2 6  Prescribed circumstancetesting the market - Abrievated Graph Key: I20"@en-AU ;
    skos:definition "2 6  Prescribed circumstancetesting the market"@en-AU ;
    skos:narrower F2021L00312:10 ;
    skos:prefLabel "Item I20"@en-AU ;
    dcat:accessURL <https://www.legislation.gov.au/F2021L00312/asmade/2021-03-24/text/original/epub/OEBPS/document_1/document_1.html#_Toc65843304> ;
    dcat:landingPage "https://www.legislation.gov.au/F2021L00312/asmade/2021-03-24/text/original/epub/OEBPS/document_1/document_1.html#_Toc65843304"^^xsd:anyURI ;
    dcat:theme legcons:Item .

F2021L00312:200 a legcons:Item,
        owl:Class,
        dcat:Resource ;
    rdfs:label "Item - I200 9 12  Notice of decision"@en-AU ;
    dct:isPartOf F2021L00312:194 ;
    dct:isReferencedBy F2021L00312: ;
    rdfs:comment "9 12  Notice of decision - Abrievated Graph Key: I200"@en-AU ;
    skos:definition "9 12  Notice of decision"@en-AU ;
    skos:narrower F2021L00312:194 ;
    skos:prefLabel "Item I200"@en-AU ;
    dcat:accessURL <https://www.legislation.gov.au/F2021L00312/asmade/2021-03-24/text/original/epub/OEBPS/document_1/document_1.html#_Toc65843484> ;
    dcat:landingPage "https://www.legislation.gov.au/F2021L00312/asmade/2021-03-24/text/original/epub/OEBPS/document_1/document_1.html#_Toc65843484"^^xsd:anyURI ;
    dcat:theme legcons:Item .

F2021L00312:201 a legcons:Item,
        owl:Class,
        dcat:Resource ;
    rdfs:label "Item - I201 9 13  Period of effect of approval"@en-AU ;
    dct:isPartOf F2021L00312:194 ;
    dct:isReferencedBy F2021L00312: ;
    rdfs:comment "9 13  Period of effect of approval - Abrievated Graph Key: I201"@en-AU ;
    skos:definition "9 13  Period of effect of approval"@en-AU ;
    skos:narrower F2021L00312:194 ;
    skos:prefLabel "Item I201"@en-AU ;
    dcat:accessURL <https://www.legislation.gov.au/F2021L00312/asmade/2021-03-24/text/original/epub/OEBPS/document_1/document_1.html#_Toc65843485> ;
    dcat:landingPage "https://www.legislation.gov.au/F2021L00312/asmade/2021-03-24/text/original/epub/OEBPS/document_1/document_1.html#_Toc65843485"^^xsd:anyURI ;
    dcat:theme legcons:Item .

F2021L00312:202 a legcons:Item,
        owl:Class,
        dcat:Resource ;
    rdfs:label "Item - I202 9 14  Imposing or varying conditions of approval"@en-AU ;
    dct:isPartOf F2021L00312:194 ;
    dct:isReferencedBy F2021L00312: ;
    rdfs:comment "9 14  Imposing or varying conditions of approval - Abrievated Graph Key: I202"@en-AU ;
    skos:definition "9 14  Imposing or varying conditions of approval"@en-AU ;
    skos:narrower F2021L00312:194 ;
    skos:prefLabel "Item I202"@en-AU ;
    dcat:accessURL <https://www.legislation.gov.au/F2021L00312/asmade/2021-03-24/text/original/epub/OEBPS/document_1/document_1.html#_Toc65843486> ;
    dcat:landingPage "https://www.legislation.gov.au/F2021L00312/asmade/2021-03-24/text/original/epub/OEBPS/document_1/document_1.html#_Toc65843486"^^xsd:anyURI ;
    dcat:theme legcons:Item .

F2021L00312:203 a legcons:Item,
        owl:Class,
        dcat:Resource ;
    rdfs:label "Item - I203 9 15  Revocation of approval"@en-AU ;
    dct:isPartOf F2021L00312:194 ;
    dct:isReferencedBy F2021L00312: ;
    rdfs:comment "9 15  Revocation of approval - Abrievated Graph Key: I203"@en-AU ;
    skos:definition "9 15  Revocation of approval"@en-AU ;
    skos:narrower F2021L00312:194 ;
    skos:prefLabel "Item I203"@en-AU ;
    dcat:accessURL <https://www.legislation.gov.au/F2021L00312/asmade/2021-03-24/text/original/epub/OEBPS/document_1/document_1.html#_Toc65843487> ;
    dcat:landingPage "https://www.legislation.gov.au/F2021L00312/asmade/2021-03-24/text/original/epub/OEBPS/document_1/document_1.html#_Toc65843487"^^xsd:anyURI ;
    dcat:theme legcons:Item .

F2021L00312:204 a legcons:Item,
        owl:Class,
        dcat:Resource ;
    rdfs:label "Item - I204 9 16  Register of approved auditors"@en-AU ;
    dct:isPartOf F2021L00312:194 ;
    dct:isReferencedBy F2021L00312: ;
    rdfs:comment "9 16  Register of approved auditors - Abrievated Graph Key: I204"@en-AU ;
    skos:definition "9 16  Register of approved auditors"@en-AU ;
    skos:narrower F2021L00312:194 ;
    skos:prefLabel "Item I204"@en-AU ;
    dcat:accessURL <https://www.legislation.gov.au/F2021L00312/asmade/2021-03-24/text/original/epub/OEBPS/document_1/document_1.html#_Toc65843488> ;
    dcat:landingPage "https://www.legislation.gov.au/F2021L00312/asmade/2021-03-24/text/original/epub/OEBPS/document_1/document_1.html#_Toc65843488"^^xsd:anyURI ;
    dcat:theme legcons:Item .

F2021L00312:205 a legcons:Item,
        owl:Class,
        dcat:Resource ;
    rdfs:label "Item - I205 9 17  Fit and proper person test"@en-AU ;
    dct:isPartOf F2021L00312:194 ;
    dct:isReferencedBy F2021L00312: ;
    rdfs:comment "9 17  Fit and proper person test - Abrievated Graph Key: I205"@en-AU ;
    skos:definition "9 17  Fit and proper person test"@en-AU ;
    skos:narrower F2021L00312:194 ;
    skos:prefLabel "Item I205"@en-AU ;
    dcat:accessURL <https://www.legislation.gov.au/F2021L00312/asmade/2021-03-24/text/original/epub/OEBPS/document_1/document_1.html#_Toc65843489> ;
    dcat:landingPage "https://www.legislation.gov.au/F2021L00312/asmade/2021-03-24/text/original/epub/OEBPS/document_1/document_1.html#_Toc65843489"^^xsd:anyURI ;
    dcat:theme legcons:Item .

F2021L00312:208 a legcons:Item,
        owl:Class,
        dcat:Resource ;
    rdfs:label "Item - I208 9 18  References to assessment in this Part"@en-AU ;
    dct:isPartOf F2021L00312:207 ;
    dct:isReferencedBy F2021L00312: ;
    rdfs:comment "9 18  References to assessment in this Part - Abrievated Graph Key: I208"@en-AU ;
    skos:definition "9 18  References to assessment in this Part"@en-AU ;
    skos:narrower F2021L00312:207 ;
    skos:prefLabel "Item I208"@en-AU ;
    dcat:accessURL <https://www.legislation.gov.au/F2021L00312/asmade/2021-03-24/text/original/epub/OEBPS/document_1/document_1.html#_Toc65843492> ;
    dcat:landingPage "https://www.legislation.gov.au/F2021L00312/asmade/2021-03-24/text/original/epub/OEBPS/document_1/document_1.html#_Toc65843492"^^xsd:anyURI ;
    dcat:theme legcons:Item .

F2021L00312:21 a legcons:Item,
        owl:Class,
        dcat:Resource ;
    rdfs:label "Item - I21 2 7  Prescribed meaningcommercial sample"@en-AU ;
    dct:isPartOf F2021L00312:10 ;
    dct:isReferencedBy F2021L00312: ;
    rdfs:comment "2 7  Prescribed meaningcommercial sample - Abrievated Graph Key: I21"@en-AU ;
    skos:definition "2 7  Prescribed meaningcommercial sample"@en-AU ;
    skos:narrower F2021L00312:10 ;
    skos:prefLabel "Item I21"@en-AU ;
    dcat:accessURL <https://www.legislation.gov.au/F2021L00312/asmade/2021-03-24/text/original/epub/OEBPS/document_1/document_1.html#_Toc65843305> ;
    dcat:landingPage "https://www.legislation.gov.au/F2021L00312/asmade/2021-03-24/text/original/epub/OEBPS/document_1/document_1.html#_Toc65843305"^^xsd:anyURI ;
    dcat:theme legcons:Item .

F2021L00312:210 a legcons:Item,
        owl:Class,
        dcat:Resource ;
    rdfs:label "Item - I210 9 19  Circumstances in which assessment may be required or permitted"@en-AU ;
    dct:isPartOf F2021L00312:209 ;
    dct:isReferencedBy F2021L00312: ;
    rdfs:comment "9 19  Circumstances in which assessment may be required or permitted - Abrievated Graph Key: I210"@en-AU ;
    skos:definition "9 19  Circumstances in which assessment may be required or permitted"@en-AU ;
    skos:narrower F2021L00312:209 ;
    skos:prefLabel "Item I210"@en-AU ;
    dcat:accessURL <https://www.legislation.gov.au/F2021L00312/asmade/2021-03-24/text/original/epub/OEBPS/document_1/document_1.html#_Toc65843494> ;
    dcat:landingPage "https://www.legislation.gov.au/F2021L00312/asmade/2021-03-24/text/original/epub/OEBPS/document_1/document_1.html#_Toc65843494"^^xsd:anyURI ;
    dcat:theme legcons:Item .

F2021L00312:211 a legcons:Item,
        owl:Class,
        dcat:Resource ;
    rdfs:label "Item - I211 9 20  Process to be followed after assessment completed"@en-AU ;
    dct:isPartOf F2021L00312:209 ;
    dct:isReferencedBy F2021L00312: ;
    rdfs:comment "9 20  Process to be followed after assessment completed - Abrievated Graph Key: I211"@en-AU ;
    skos:definition "9 20  Process to be followed after assessment completed"@en-AU ;
    skos:narrower F2021L00312:209 ;
    skos:prefLabel "Item I211"@en-AU ;
    dcat:accessURL <https://www.legislation.gov.au/F2021L00312/asmade/2021-03-24/text/original/epub/OEBPS/document_1/document_1.html#_Toc65843495> ;
    dcat:landingPage "https://www.legislation.gov.au/F2021L00312/asmade/2021-03-24/text/original/epub/OEBPS/document_1/document_1.html#_Toc65843495"^^xsd:anyURI ;
    dcat:theme legcons:Item .

F2021L00312:213 a legcons:Item,
        owl:Class,
        dcat:Resource ;
    rdfs:label "Item - I213 9 21  Purpose of this Division"@en-AU ;
    dct:isPartOf F2021L00312:212 ;
    dct:isReferencedBy F2021L00312: ;
    rdfs:comment "9 21  Purpose of this Division - Abrievated Graph Key: I213"@en-AU ;
    skos:definition "9 21  Purpose of this Division"@en-AU ;
    skos:narrower F2021L00312:212 ;
    skos:prefLabel "Item I213"@en-AU ;
    dcat:accessURL <https://www.legislation.gov.au/F2021L00312/asmade/2021-03-24/text/original/epub/OEBPS/document_1/document_1.html#_Toc65843497> ;
    dcat:landingPage "https://www.legislation.gov.au/F2021L00312/asmade/2021-03-24/text/original/epub/OEBPS/document_1/document_1.html#_Toc65843497"^^xsd:anyURI ;
    dcat:theme legcons:Item .

F2021L00312:214 a legcons:Item,
        owl:Class,
        dcat:Resource ;
    rdfs:label "Item - I214 9 22  Application for approval"@en-AU ;
    dct:isPartOf F2021L00312:212 ;
    dct:isReferencedBy F2021L00312: ;
    rdfs:comment "9 22  Application for approval - Abrievated Graph Key: I214"@en-AU ;
    skos:definition "9 22  Application for approval"@en-AU ;
    skos:narrower F2021L00312:212 ;
    skos:prefLabel "Item I214"@en-AU ;
    dcat:accessURL <https://www.legislation.gov.au/F2021L00312/asmade/2021-03-24/text/original/epub/OEBPS/document_1/document_1.html#_Toc65843498> ;
    dcat:landingPage "https://www.legislation.gov.au/F2021L00312/asmade/2021-03-24/text/original/epub/OEBPS/document_1/document_1.html#_Toc65843498"^^xsd:anyURI ;
    dcat:theme legcons:Item .

F2021L00312:215 a legcons:Item,
        owl:Class,
        dcat:Resource ;
    rdfs:label "Item - I215 9 23  Secretary must decide whether to approve applicant to carry out assessments"@en-AU ;
    dct:isPartOf F2021L00312:212 ;
    dct:isReferencedBy F2021L00312: ;
    rdfs:comment "9 23  Secretary must decide whether to approve applicant to carry out assessments - Abrievated Graph Key: I215"@en-AU ;
    skos:definition "9 23  Secretary must decide whether to approve applicant to carry out assessments"@en-AU ;
    skos:narrower F2021L00312:212 ;
    skos:prefLabel "Item I215"@en-AU ;
    dcat:accessURL <https://www.legislation.gov.au/F2021L00312/asmade/2021-03-24/text/original/epub/OEBPS/document_1/document_1.html#_Toc65843499> ;
    dcat:landingPage "https://www.legislation.gov.au/F2021L00312/asmade/2021-03-24/text/original/epub/OEBPS/document_1/document_1.html#_Toc65843499"^^xsd:anyURI ;
    dcat:theme legcons:Item .

F2021L00312:216 a legcons:Item,
        owl:Class,
        dcat:Resource ;
    rdfs:label "Item - I216 9 24  Dealing with applications"@en-AU ;
    dct:isPartOf F2021L00312:212 ;
    dct:isReferencedBy F2021L00312: ;
    rdfs:comment "9 24  Dealing with applications - Abrievated Graph Key: I216"@en-AU ;
    skos:definition "9 24  Dealing with applications"@en-AU ;
    skos:narrower F2021L00312:212 ;
    skos:prefLabel "Item I216"@en-AU ;
    dcat:accessURL <https://www.legislation.gov.au/F2021L00312/asmade/2021-03-24/text/original/epub/OEBPS/document_1/document_1.html#_Toc65843500> ;
    dcat:landingPage "https://www.legislation.gov.au/F2021L00312/asmade/2021-03-24/text/original/epub/OEBPS/document_1/document_1.html#_Toc65843500"^^xsd:anyURI ;
    dcat:theme legcons:Item .

F2021L00312:217 a legcons:Item,
        owl:Class,
        dcat:Resource ;
    rdfs:label "Item - I217 9 25  Conditions of approval"@en-AU ;
    dct:isPartOf F2021L00312:212 ;
    dct:isReferencedBy F2021L00312: ;
    rdfs:comment "9 25  Conditions of approval - Abrievated Graph Key: I217"@en-AU ;
    skos:definition "9 25  Conditions of approval"@en-AU ;
    skos:narrower F2021L00312:212 ;
    skos:prefLabel "Item I217"@en-AU ;
    dcat:accessURL <https://www.legislation.gov.au/F2021L00312/asmade/2021-03-24/text/original/epub/OEBPS/document_1/document_1.html#_Toc65843501> ;
    dcat:landingPage "https://www.legislation.gov.au/F2021L00312/asmade/2021-03-24/text/original/epub/OEBPS/document_1/document_1.html#_Toc65843501"^^xsd:anyURI ;
    dcat:theme legcons:Item .

F2021L00312:218 a legcons:Item,
        owl:Class,
        dcat:Resource ;
    rdfs:label "Item - I218 9 26  Notice of decision"@en-AU ;
    dct:isPartOf F2021L00312:212 ;
    dct:isReferencedBy F2021L00312: ;
    rdfs:comment "9 26  Notice of decision - Abrievated Graph Key: I218"@en-AU ;
    skos:definition "9 26  Notice of decision"@en-AU ;
    skos:narrower F2021L00312:212 ;
    skos:prefLabel "Item I218"@en-AU ;
    dcat:accessURL <https://www.legislation.gov.au/F2021L00312/asmade/2021-03-24/text/original/epub/OEBPS/document_1/document_1.html#_Toc65843502> ;
    dcat:landingPage "https://www.legislation.gov.au/F2021L00312/asmade/2021-03-24/text/original/epub/OEBPS/document_1/document_1.html#_Toc65843502"^^xsd:anyURI ;
    dcat:theme legcons:Item .

F2021L00312:219 a legcons:Item,
        owl:Class,
        dcat:Resource ;
    rdfs:label "Item - I219 9 27  Period of effect of approval"@en-AU ;
    dct:isPartOf F2021L00312:212 ;
    dct:isReferencedBy F2021L00312: ;
    rdfs:comment "9 27  Period of effect of approval - Abrievated Graph Key: I219"@en-AU ;
    skos:definition "9 27  Period of effect of approval"@en-AU ;
    skos:narrower F2021L00312:212 ;
    skos:prefLabel "Item I219"@en-AU ;
    dcat:accessURL <https://www.legislation.gov.au/F2021L00312/asmade/2021-03-24/text/original/epub/OEBPS/document_1/document_1.html#_Toc65843503> ;
    dcat:landingPage "https://www.legislation.gov.au/F2021L00312/asmade/2021-03-24/text/original/epub/OEBPS/document_1/document_1.html#_Toc65843503"^^xsd:anyURI ;
    dcat:theme legcons:Item .

F2021L00312:22 a legcons:Item,
        owl:Class,
        dcat:Resource ;
    rdfs:label "Item - I22 2 8  Period for making application for exemption"@en-AU ;
    dct:isPartOf F2021L00312:10 ;
    dct:isReferencedBy F2021L00312: ;
    rdfs:comment "2 8  Period for making application for exemption - Abrievated Graph Key: I22"@en-AU ;
    skos:definition "2 8  Period for making application for exemption"@en-AU ;
    skos:narrower F2021L00312:10 ;
    skos:prefLabel "Item I22"@en-AU ;
    dcat:accessURL <https://www.legislation.gov.au/F2021L00312/asmade/2021-03-24/text/original/epub/OEBPS/document_1/document_1.html#_Toc65843306> ;
    dcat:landingPage "https://www.legislation.gov.au/F2021L00312/asmade/2021-03-24/text/original/epub/OEBPS/document_1/document_1.html#_Toc65843306"^^xsd:anyURI ;
    dcat:theme legcons:Item .

F2021L00312:220 a legcons:Item,
        owl:Class,
        dcat:Resource ;
    rdfs:label "Item - I220 9 28  Imposing or varying conditions of approval"@en-AU ;
    dct:isPartOf F2021L00312:212 ;
    dct:isReferencedBy F2021L00312: ;
    rdfs:comment "9 28  Imposing or varying conditions of approval - Abrievated Graph Key: I220"@en-AU ;
    skos:definition "9 28  Imposing or varying conditions of approval"@en-AU ;
    skos:narrower F2021L00312:212 ;
    skos:prefLabel "Item I220"@en-AU ;
    dcat:accessURL <https://www.legislation.gov.au/F2021L00312/asmade/2021-03-24/text/original/epub/OEBPS/document_1/document_1.html#_Toc65843504> ;
    dcat:landingPage "https://www.legislation.gov.au/F2021L00312/asmade/2021-03-24/text/original/epub/OEBPS/document_1/document_1.html#_Toc65843504"^^xsd:anyURI ;
    dcat:theme legcons:Item .

F2021L00312:221 a legcons:Item,
        owl:Class,
        dcat:Resource ;
    rdfs:label "Item - I221 9 29  Revocation of approval"@en-AU ;
    dct:isPartOf F2021L00312:212 ;
    dct:isReferencedBy F2021L00312: ;
    rdfs:comment "9 29  Revocation of approval - Abrievated Graph Key: I221"@en-AU ;
    skos:definition "9 29  Revocation of approval"@en-AU ;
    skos:narrower F2021L00312:212 ;
    skos:prefLabel "Item I221"@en-AU ;
    dcat:accessURL <https://www.legislation.gov.au/F2021L00312/asmade/2021-03-24/text/original/epub/OEBPS/document_1/document_1.html#_Toc65843505> ;
    dcat:landingPage "https://www.legislation.gov.au/F2021L00312/asmade/2021-03-24/text/original/epub/OEBPS/document_1/document_1.html#_Toc65843505"^^xsd:anyURI ;
    dcat:theme legcons:Item .

F2021L00312:222 a legcons:Item,
        owl:Class,
        dcat:Resource ;
    rdfs:label "Item - I222 9 30  Register of approved assessors"@en-AU ;
    dct:isPartOf F2021L00312:212 ;
    dct:isReferencedBy F2021L00312: ;
    rdfs:comment "9 30  Register of approved assessors - Abrievated Graph Key: I222"@en-AU ;
    skos:definition "9 30  Register of approved assessors"@en-AU ;
    skos:narrower F2021L00312:212 ;
    skos:prefLabel "Item I222"@en-AU ;
    dcat:accessURL <https://www.legislation.gov.au/F2021L00312/asmade/2021-03-24/text/original/epub/OEBPS/document_1/document_1.html#_Toc65843506> ;
    dcat:landingPage "https://www.legislation.gov.au/F2021L00312/asmade/2021-03-24/text/original/epub/OEBPS/document_1/document_1.html#_Toc65843506"^^xsd:anyURI ;
    dcat:theme legcons:Item .

F2021L00312:223 a legcons:Item,
        owl:Class,
        dcat:Resource ;
    rdfs:label "Item - I223 9 31  Fit and proper person test"@en-AU ;
    dct:isPartOf F2021L00312:212 ;
    dct:isReferencedBy F2021L00312: ;
    rdfs:comment "9 31  Fit and proper person test - Abrievated Graph Key: I223"@en-AU ;
    skos:definition "9 31  Fit and proper person test"@en-AU ;
    skos:narrower F2021L00312:212 ;
    skos:prefLabel "Item I223"@en-AU ;
    dcat:accessURL <https://www.legislation.gov.au/F2021L00312/asmade/2021-03-24/text/original/epub/OEBPS/document_1/document_1.html#_Toc65843507> ;
    dcat:landingPage "https://www.legislation.gov.au/F2021L00312/asmade/2021-03-24/text/original/epub/OEBPS/document_1/document_1.html#_Toc65843507"^^xsd:anyURI ;
    dcat:theme legcons:Item .

F2021L00312:225 a legcons:Item,
        owl:Class,
        dcat:Resource ;
    rdfs:label "Item - I225 9 32  Decisions that may be made by operation of computer program"@en-AU ;
    dct:isPartOf F2021L00312:224 ;
    dct:isReferencedBy F2021L00312: ;
    rdfs:comment "9 32  Decisions that may be made by operation of computer program - Abrievated Graph Key: I225"@en-AU ;
    skos:definition "9 32  Decisions that may be made by operation of computer program"@en-AU ;
    skos:narrower F2021L00312:224 ;
    skos:prefLabel "Item I225"@en-AU ;
    dcat:accessURL <https://www.legislation.gov.au/F2021L00312/asmade/2021-03-24/text/original/epub/OEBPS/document_1/document_1.html#_Toc65843509> ;
    dcat:landingPage "https://www.legislation.gov.au/F2021L00312/asmade/2021-03-24/text/original/epub/OEBPS/document_1/document_1.html#_Toc65843509"^^xsd:anyURI ;
    dcat:theme legcons:Item .

F2021L00312:228 a legcons:Item,
        owl:Class,
        dcat:Resource ;
    rdfs:label "Item - I228 9 33  Requirement to be third party authorised officerfit and proper person etc"@en-AU ;
    dct:isPartOf F2021L00312:227 ;
    dct:isReferencedBy F2021L00312: ;
    rdfs:comment "9 33  Requirement to be third party authorised officerfit and proper person etc - Abrievated Graph Key: I228"@en-AU ;
    skos:definition "9 33  Requirement to be third party authorised officerfit and proper person etc"@en-AU ;
    skos:narrower F2021L00312:227 ;
    skos:prefLabel "Item I228"@en-AU ;
    dcat:accessURL <https://www.legislation.gov.au/F2021L00312/asmade/2021-03-24/text/original/epub/OEBPS/document_1/document_1.html#_Toc65843512> ;
    dcat:landingPage "https://www.legislation.gov.au/F2021L00312/asmade/2021-03-24/text/original/epub/OEBPS/document_1/document_1.html#_Toc65843512"^^xsd:anyURI ;
    dcat:theme legcons:Item .

F2021L00312:23 a legcons:Item,
        owl:Class,
        dcat:Resource ;
    rdfs:label "Item - I23 2 9  Conditions of exemptionmatters to which Secretary must have regard"@en-AU ;
    dct:isPartOf F2021L00312:10 ;
    dct:isReferencedBy F2021L00312: ;
    rdfs:comment "2 9  Conditions of exemptionmatters to which Secretary must have regard - Abrievated Graph Key: I23"@en-AU ;
    skos:definition "2 9  Conditions of exemptionmatters to which Secretary must have regard"@en-AU ;
    skos:narrower F2021L00312:10 ;
    skos:prefLabel "Item I23"@en-AU ;
    dcat:accessURL <https://www.legislation.gov.au/F2021L00312/asmade/2021-03-24/text/original/epub/OEBPS/document_1/document_1.html#_Toc65843307> ;
    dcat:landingPage "https://www.legislation.gov.au/F2021L00312/asmade/2021-03-24/text/original/epub/OEBPS/document_1/document_1.html#_Toc65843307"^^xsd:anyURI ;
    dcat:theme legcons:Item .

F2021L00312:230 a legcons:Item,
        owl:Class,
        dcat:Resource ;
    rdfs:label "Item - I230 9 34  Purpose of this Division"@en-AU ;
    dct:isPartOf F2021L00312:229 ;
    dct:isReferencedBy F2021L00312: ;
    rdfs:comment "9 34  Purpose of this Division - Abrievated Graph Key: I230"@en-AU ;
    skos:definition "9 34  Purpose of this Division"@en-AU ;
    skos:narrower F2021L00312:229 ;
    skos:prefLabel "Item I230"@en-AU ;
    dcat:accessURL <https://www.legislation.gov.au/F2021L00312/asmade/2021-03-24/text/original/epub/OEBPS/document_1/document_1.html#_Toc65843514> ;
    dcat:landingPage "https://www.legislation.gov.au/F2021L00312/asmade/2021-03-24/text/original/epub/OEBPS/document_1/document_1.html#_Toc65843514"^^xsd:anyURI ;
    dcat:theme legcons:Item .

F2021L00312:231 a legcons:Item,
        owl:Class,
        dcat:Resource ;
    rdfs:label "Item - I231 9 35  Inspecting establishments and securing areas facilities equipment or other things"@en-AU ;
    dct:isPartOf F2021L00312:229 ;
    dct:isReferencedBy F2021L00312: ;
    rdfs:comment "9 35  Inspecting establishments and securing areas facilities equipment or other things - Abrievated Graph Key: I231"@en-AU ;
    skos:definition "9 35  Inspecting establishments and securing areas facilities equipment or other things"@en-AU ;
    skos:narrower F2021L00312:229 ;
    skos:prefLabel "Item I231"@en-AU ;
    dcat:accessURL <https://www.legislation.gov.au/F2021L00312/asmade/2021-03-24/text/original/epub/OEBPS/document_1/document_1.html#_Toc65843515> ;
    dcat:landingPage "https://www.legislation.gov.au/F2021L00312/asmade/2021-03-24/text/original/epub/OEBPS/document_1/document_1.html#_Toc65843515"^^xsd:anyURI ;
    dcat:theme legcons:Item .

F2021L00312:232 a legcons:Item,
        owl:Class,
        dcat:Resource ;
    rdfs:label "Item - I232 9 36  Securing and identifying establishment or conveyance etc"@en-AU ;
    dct:isPartOf F2021L00312:229 ;
    dct:isReferencedBy F2021L00312: ;
    rdfs:comment "9 36  Securing and identifying establishment or conveyance etc - Abrievated Graph Key: I232"@en-AU ;
    skos:definition "9 36  Securing and identifying establishment or conveyance etc"@en-AU ;
    skos:narrower F2021L00312:229 ;
    skos:prefLabel "Item I232"@en-AU ;
    dcat:accessURL <https://www.legislation.gov.au/F2021L00312/asmade/2021-03-24/text/original/epub/OEBPS/document_1/document_1.html#_Toc65843516> ;
    dcat:landingPage "https://www.legislation.gov.au/F2021L00312/asmade/2021-03-24/text/original/epub/OEBPS/document_1/document_1.html#_Toc65843516"^^xsd:anyURI ;
    dcat:theme legcons:Item .

F2021L00312:233 a legcons:Item,
        owl:Class,
        dcat:Resource ;
    rdfs:label "Item - I233 9 37  Interference with identified establishment or conveyance etc"@en-AU ;
    dct:isPartOf F2021L00312:229 ;
    dct:isReferencedBy F2021L00312: ;
    rdfs:comment "9 37  Interference with identified establishment or conveyance etc - Abrievated Graph Key: I233"@en-AU ;
    skos:definition "9 37  Interference with identified establishment or conveyance etc"@en-AU ;
    skos:narrower F2021L00312:229 ;
    skos:prefLabel "Item I233"@en-AU ;
    dcat:accessURL <https://www.legislation.gov.au/F2021L00312/asmade/2021-03-24/text/original/epub/OEBPS/document_1/document_1.html#_Toc65843517> ;
    dcat:landingPage "https://www.legislation.gov.au/F2021L00312/asmade/2021-03-24/text/original/epub/OEBPS/document_1/document_1.html#_Toc65843517"^^xsd:anyURI ;
    dcat:theme legcons:Item .

F2021L00312:235 a legcons:Item,
        owl:Class,
        dcat:Resource ;
    rdfs:label "Item - I235 9 38  Other grounds for giving direction"@en-AU ;
    dct:isPartOf F2021L00312:234 ;
    dct:isReferencedBy F2021L00312: ;
    rdfs:comment "9 38  Other grounds for giving direction - Abrievated Graph Key: I235"@en-AU ;
    skos:definition "9 38  Other grounds for giving direction"@en-AU ;
    skos:narrower F2021L00312:234 ;
    skos:prefLabel "Item I235"@en-AU ;
    dcat:accessURL <https://www.legislation.gov.au/F2021L00312/asmade/2021-03-24/text/original/epub/OEBPS/document_1/document_1.html#_Toc65843519> ;
    dcat:landingPage "https://www.legislation.gov.au/F2021L00312/asmade/2021-03-24/text/original/epub/OEBPS/document_1/document_1.html#_Toc65843519"^^xsd:anyURI ;
    dcat:theme legcons:Item .

F2021L00312:237 a legcons:Item,
        owl:Class,
        dcat:Resource ;
    rdfs:label "Item - I237 9 39  Circumstances in which identity card need not be carried"@en-AU ;
    dct:isPartOf F2021L00312:236 ;
    dct:isReferencedBy F2021L00312: ;
    rdfs:comment "9 39  Circumstances in which identity card need not be carried - Abrievated Graph Key: I237"@en-AU ;
    skos:definition "9 39  Circumstances in which identity card need not be carried"@en-AU ;
    skos:narrower F2021L00312:236 ;
    skos:prefLabel "Item I237"@en-AU ;
    dcat:accessURL <https://www.legislation.gov.au/F2021L00312/asmade/2021-03-24/text/original/epub/OEBPS/document_1/document_1.html#_Toc65843521> ;
    dcat:landingPage "https://www.legislation.gov.au/F2021L00312/asmade/2021-03-24/text/original/epub/OEBPS/document_1/document_1.html#_Toc65843521"^^xsd:anyURI ;
    dcat:theme legcons:Item .

F2021L00312:239 a legcons:Item,
        owl:Class,
        dcat:Resource ;
    rdfs:label "Item - I239 10 1  Samples taken in exercising monitoring or investigation powers"@en-AU ;
    dct:isPartOf F2021L00312:238 ;
    dct:isReferencedBy F2021L00312: ;
    rdfs:comment "10 1  Samples taken in exercising monitoring or investigation powers - Abrievated Graph Key: I239"@en-AU ;
    skos:definition "10 1  Samples taken in exercising monitoring or investigation powers"@en-AU ;
    skos:narrower F2021L00312:238 ;
    skos:prefLabel "Item I239"@en-AU ;
    dcat:accessURL <https://www.legislation.gov.au/F2021L00312/asmade/2021-03-24/text/original/epub/OEBPS/document_1/document_1.html#_Toc65843523> ;
    dcat:landingPage "https://www.legislation.gov.au/F2021L00312/asmade/2021-03-24/text/original/epub/OEBPS/document_1/document_1.html#_Toc65843523"^^xsd:anyURI ;
    dcat:theme legcons:Item .

F2021L00312:24 a legcons:Item,
        owl:Class,
        dcat:Resource ;
    rdfs:label "Item - I24 2 10  Instrument of exemption"@en-AU ;
    dct:isPartOf F2021L00312:10 ;
    dct:isReferencedBy F2021L00312: ;
    rdfs:comment "2 10  Instrument of exemption - Abrievated Graph Key: I24"@en-AU ;
    skos:definition "2 10  Instrument of exemption"@en-AU ;
    skos:narrower F2021L00312:10 ;
    skos:prefLabel "Item I24"@en-AU ;
    dcat:accessURL <https://www.legislation.gov.au/F2021L00312/asmade/2021-03-24/text/original/epub/OEBPS/document_1/document_1.html#_Toc65843308> ;
    dcat:landingPage "https://www.legislation.gov.au/F2021L00312/asmade/2021-03-24/text/original/epub/OEBPS/document_1/document_1.html#_Toc65843308"^^xsd:anyURI ;
    dcat:theme legcons:Item .

F2021L00312:240 a legcons:Item,
        owl:Class,
        dcat:Resource ;
    rdfs:label "Item - I240 10 2  Dealing with things seized in exercising investigation powers"@en-AU ;
    dct:isPartOf F2021L00312:238 ;
    dct:isReferencedBy F2021L00312: ;
    rdfs:comment "10 2  Dealing with things seized in exercising investigation powers - Abrievated Graph Key: I240"@en-AU ;
    skos:definition "10 2  Dealing with things seized in exercising investigation powers"@en-AU ;
    skos:narrower F2021L00312:238 ;
    skos:prefLabel "Item I240"@en-AU ;
    dcat:accessURL <https://www.legislation.gov.au/F2021L00312/asmade/2021-03-24/text/original/epub/OEBPS/document_1/document_1.html#_Toc65843524> ;
    dcat:landingPage "https://www.legislation.gov.au/F2021L00312/asmade/2021-03-24/text/original/epub/OEBPS/document_1/document_1.html#_Toc65843524"^^xsd:anyURI ;
    dcat:theme legcons:Item .

F2021L00312:243 a legcons:Item,
        owl:Class,
        dcat:Resource ;
    rdfs:label "Item - I243 11 1  Reviewable decisions"@en-AU ;
    dct:isPartOf F2021L00312:242 ;
    dct:isReferencedBy F2021L00312: ;
    rdfs:comment "11 1  Reviewable decisions - Abrievated Graph Key: I243"@en-AU ;
    skos:definition "11 1  Reviewable decisions"@en-AU ;
    skos:narrower F2021L00312:242 ;
    skos:prefLabel "Item I243"@en-AU ;
    dcat:accessURL <https://www.legislation.gov.au/F2021L00312/asmade/2021-03-24/text/original/epub/OEBPS/document_1/document_1.html#_Toc65843527> ;
    dcat:landingPage "https://www.legislation.gov.au/F2021L00312/asmade/2021-03-24/text/original/epub/OEBPS/document_1/document_1.html#_Toc65843527"^^xsd:anyURI ;
    dcat:theme legcons:Item .

F2021L00312:245 a legcons:Item,
        owl:Class,
        dcat:Resource ;
    rdfs:label "Item - I245 11 2  Purpose of this Part"@en-AU ;
    dct:isPartOf F2021L00312:244 ;
    dct:isReferencedBy F2021L00312: ;
    rdfs:comment "11 2  Purpose of this Part - Abrievated Graph Key: I245"@en-AU ;
    skos:definition "11 2  Purpose of this Part"@en-AU ;
    skos:narrower F2021L00312:244 ;
    skos:prefLabel "Item I245"@en-AU ;
    dcat:accessURL <https://www.legislation.gov.au/F2021L00312/asmade/2021-03-24/text/original/epub/OEBPS/document_1/document_1.html#_Toc65843529> ;
    dcat:landingPage "https://www.legislation.gov.au/F2021L00312/asmade/2021-03-24/text/original/epub/OEBPS/document_1/document_1.html#_Toc65843529"^^xsd:anyURI ;
    dcat:theme legcons:Item .

F2021L00312:246 a legcons:Item,
        owl:Class,
        dcat:Resource ;
    rdfs:label "Item - I246 11 3  General requirements for records"@en-AU ;
    dct:isPartOf F2021L00312:244 ;
    dct:isReferencedBy F2021L00312: ;
    rdfs:comment "11 3  General requirements for records - Abrievated Graph Key: I246"@en-AU ;
    skos:definition "11 3  General requirements for records"@en-AU ;
    skos:narrower F2021L00312:244 ;
    skos:prefLabel "Item I246"@en-AU ;
    dcat:accessURL <https://www.legislation.gov.au/F2021L00312/asmade/2021-03-24/text/original/epub/OEBPS/document_1/document_1.html#_Toc65843530> ;
    dcat:landingPage "https://www.legislation.gov.au/F2021L00312/asmade/2021-03-24/text/original/epub/OEBPS/document_1/document_1.html#_Toc65843530"^^xsd:anyURI ;
    dcat:theme legcons:Item .

F2021L00312:247 a legcons:Item,
        owl:Class,
        dcat:Resource ;
    rdfs:label "Item - I247 11 4  Government certificates"@en-AU ;
    dct:isPartOf F2021L00312:244 ;
    dct:isReferencedBy F2021L00312: ;
    rdfs:comment "11 4  Government certificates - Abrievated Graph Key: I247"@en-AU ;
    skos:definition "11 4  Government certificates"@en-AU ;
    skos:narrower F2021L00312:244 ;
    skos:prefLabel "Item I247"@en-AU ;
    dcat:accessURL <https://www.legislation.gov.au/F2021L00312/asmade/2021-03-24/text/original/epub/OEBPS/document_1/document_1.html#_Toc65843531> ;
    dcat:landingPage "https://www.legislation.gov.au/F2021L00312/asmade/2021-03-24/text/original/epub/OEBPS/document_1/document_1.html#_Toc65843531"^^xsd:anyURI ;
    dcat:theme legcons:Item .

F2021L00312:248 a legcons:Item,
        owl:Class,
        dcat:Resource ;
    rdfs:label "Item - I248 11 5  Export permits"@en-AU ;
    dct:isPartOf F2021L00312:244 ;
    dct:isReferencedBy F2021L00312: ;
    rdfs:comment "11 5  Export permits - Abrievated Graph Key: I248"@en-AU ;
    skos:definition "11 5  Export permits"@en-AU ;
    skos:narrower F2021L00312:244 ;
    skos:prefLabel "Item I248"@en-AU ;
    dcat:accessURL <https://www.legislation.gov.au/F2021L00312/asmade/2021-03-24/text/original/epub/OEBPS/document_1/document_1.html#_Toc65843532> ;
    dcat:landingPage "https://www.legislation.gov.au/F2021L00312/asmade/2021-03-24/text/original/epub/OEBPS/document_1/document_1.html#_Toc65843532"^^xsd:anyURI ;
    dcat:theme legcons:Item .

F2021L00312:249 a legcons:Item,
        owl:Class,
        dcat:Resource ;
    rdfs:label "Item - I249 11 6  Records to be retained by exporter"@en-AU ;
    dct:isPartOf F2021L00312:244 ;
    dct:isReferencedBy F2021L00312: ;
    rdfs:comment "11 6  Records to be retained by exporter - Abrievated Graph Key: I249"@en-AU ;
    skos:definition "11 6  Records to be retained by exporter"@en-AU ;
    skos:narrower F2021L00312:244 ;
    skos:prefLabel "Item I249"@en-AU ;
    dcat:accessURL <https://www.legislation.gov.au/F2021L00312/asmade/2021-03-24/text/original/epub/OEBPS/document_1/document_1.html#_Toc65843533> ;
    dcat:landingPage "https://www.legislation.gov.au/F2021L00312/asmade/2021-03-24/text/original/epub/OEBPS/document_1/document_1.html#_Toc65843533"^^xsd:anyURI ;
    dcat:theme legcons:Item .

F2021L00312:25 a legcons:Item,
        owl:Class,
        dcat:Resource ;
    rdfs:label "Item - I25 2 11  Period of effect of exemption"@en-AU ;
    dct:isPartOf F2021L00312:10 ;
    dct:isReferencedBy F2021L00312: ;
    rdfs:comment "2 11  Period of effect of exemption - Abrievated Graph Key: I25"@en-AU ;
    skos:definition "2 11  Period of effect of exemption"@en-AU ;
    skos:narrower F2021L00312:10 ;
    skos:prefLabel "Item I25"@en-AU ;
    dcat:accessURL <https://www.legislation.gov.au/F2021L00312/asmade/2021-03-24/text/original/epub/OEBPS/document_1/document_1.html#_Toc65843309> ;
    dcat:landingPage "https://www.legislation.gov.au/F2021L00312/asmade/2021-03-24/text/original/epub/OEBPS/document_1/document_1.html#_Toc65843309"^^xsd:anyURI ;
    dcat:theme legcons:Item .

F2021L00312:250 a legcons:Item,
        owl:Class,
        dcat:Resource ;
    rdfs:label "Item - I250 11 7  Records to be retained by occupier of registered establishment"@en-AU ;
    dct:isPartOf F2021L00312:244 ;
    dct:isReferencedBy F2021L00312: ;
    rdfs:comment "11 7  Records to be retained by occupier of registered establishment - Abrievated Graph Key: I250"@en-AU ;
    skos:definition "11 7  Records to be retained by occupier of registered establishment"@en-AU ;
    skos:narrower F2021L00312:244 ;
    skos:prefLabel "Item I250"@en-AU ;
    dcat:accessURL <https://www.legislation.gov.au/F2021L00312/asmade/2021-03-24/text/original/epub/OEBPS/document_1/document_1.html#_Toc65843534> ;
    dcat:landingPage "https://www.legislation.gov.au/F2021L00312/asmade/2021-03-24/text/original/epub/OEBPS/document_1/document_1.html#_Toc65843534"^^xsd:anyURI ;
    dcat:theme legcons:Item .

F2021L00312:251 a legcons:Item,
        owl:Class,
        dcat:Resource ;
    rdfs:label "Item - I251 11 8  Records to be retained by holder of approved arrangement"@en-AU ;
    dct:isPartOf F2021L00312:244 ;
    dct:isReferencedBy F2021L00312: ;
    rdfs:comment "11 8  Records to be retained by holder of approved arrangement - Abrievated Graph Key: I251"@en-AU ;
    skos:definition "11 8  Records to be retained by holder of approved arrangement"@en-AU ;
    skos:narrower F2021L00312:244 ;
    skos:prefLabel "Item I251"@en-AU ;
    dcat:accessURL <https://www.legislation.gov.au/F2021L00312/asmade/2021-03-24/text/original/epub/OEBPS/document_1/document_1.html#_Toc65843535> ;
    dcat:landingPage "https://www.legislation.gov.au/F2021L00312/asmade/2021-03-24/text/original/epub/OEBPS/document_1/document_1.html#_Toc65843535"^^xsd:anyURI ;
    dcat:theme legcons:Item .

F2021L00312:252 a legcons:Item,
        owl:Class,
        dcat:Resource ;
    rdfs:label "Item - I252 11 9  Records relating to official marking devices"@en-AU ;
    dct:isPartOf F2021L00312:244 ;
    dct:isReferencedBy F2021L00312: ;
    rdfs:comment "11 9  Records relating to official marking devices - Abrievated Graph Key: I252"@en-AU ;
    skos:definition "11 9  Records relating to official marking devices"@en-AU ;
    skos:narrower F2021L00312:244 ;
    skos:prefLabel "Item I252"@en-AU ;
    dcat:accessURL <https://www.legislation.gov.au/F2021L00312/asmade/2021-03-24/text/original/epub/OEBPS/document_1/document_1.html#_Toc65843536> ;
    dcat:landingPage "https://www.legislation.gov.au/F2021L00312/asmade/2021-03-24/text/original/epub/OEBPS/document_1/document_1.html#_Toc65843536"^^xsd:anyURI ;
    dcat:theme legcons:Item .

F2021L00312:253 a legcons:Item,
        owl:Class,
        dcat:Resource ;
    rdfs:label "Item - I253 11 10  Records must not be altered or defaced during retention period"@en-AU ;
    dct:isPartOf F2021L00312:244 ;
    dct:isReferencedBy F2021L00312: ;
    rdfs:comment "11 10  Records must not be altered or defaced during retention period - Abrievated Graph Key: I253"@en-AU ;
    skos:definition "11 10  Records must not be altered or defaced during retention period"@en-AU ;
    skos:narrower F2021L00312:244 ;
    skos:prefLabel "Item I253"@en-AU ;
    dcat:accessURL <https://www.legislation.gov.au/F2021L00312/asmade/2021-03-24/text/original/epub/OEBPS/document_1/document_1.html#_Toc65843537> ;
    dcat:landingPage "https://www.legislation.gov.au/F2021L00312/asmade/2021-03-24/text/original/epub/OEBPS/document_1/document_1.html#_Toc65843537"^^xsd:anyURI ;
    dcat:theme legcons:Item .

F2021L00312:255 a legcons:Item,
        owl:Class,
        dcat:Resource ;
    rdfs:label "Item - I255 11 11  Microbiological limitstaking testing and analysing samples"@en-AU ;
    dct:isPartOf F2021L00312:254 ;
    dct:isReferencedBy F2021L00312: ;
    rdfs:comment "11 11  Microbiological limitstaking testing and analysing samples - Abrievated Graph Key: I255"@en-AU ;
    skos:definition "11 11  Microbiological limitstaking testing and analysing samples"@en-AU ;
    skos:narrower F2021L00312:254 ;
    skos:prefLabel "Item I255"@en-AU ;
    dcat:accessURL <https://www.legislation.gov.au/F2021L00312/asmade/2021-03-24/text/original/epub/OEBPS/document_1/document_1.html#_Toc65843539> ;
    dcat:landingPage "https://www.legislation.gov.au/F2021L00312/asmade/2021-03-24/text/original/epub/OEBPS/document_1/document_1.html#_Toc65843539"^^xsd:anyURI ;
    dcat:theme legcons:Item .

F2021L00312:256 a legcons:Item,
        owl:Class,
        dcat:Resource ;
    rdfs:label "Item - I256 11 12  Storage of samples"@en-AU ;
    dct:isPartOf F2021L00312:254 ;
    dct:isReferencedBy F2021L00312: ;
    rdfs:comment "11 12  Storage of samples - Abrievated Graph Key: I256"@en-AU ;
    skos:definition "11 12  Storage of samples"@en-AU ;
    skos:narrower F2021L00312:254 ;
    skos:prefLabel "Item I256"@en-AU ;
    dcat:accessURL <https://www.legislation.gov.au/F2021L00312/asmade/2021-03-24/text/original/epub/OEBPS/document_1/document_1.html#_Toc65843540> ;
    dcat:landingPage "https://www.legislation.gov.au/F2021L00312/asmade/2021-03-24/text/original/epub/OEBPS/document_1/document_1.html#_Toc65843540"^^xsd:anyURI ;
    dcat:theme legcons:Item .

F2021L00312:258 a legcons:Item,
        owl:Class,
        dcat:Resource ;
    rdfs:label "Item - I258 11 13  Division of compensation between owners"@en-AU ;
    dct:isPartOf F2021L00312:257 ;
    dct:isReferencedBy F2021L00312: ;
    rdfs:comment "11 13  Division of compensation between owners - Abrievated Graph Key: I258"@en-AU ;
    skos:definition "11 13  Division of compensation between owners"@en-AU ;
    skos:narrower F2021L00312:257 ;
    skos:prefLabel "Item I258"@en-AU ;
    dcat:accessURL <https://www.legislation.gov.au/F2021L00312/asmade/2021-03-24/text/original/epub/OEBPS/document_1/document_1.html#_Toc65843542> ;
    dcat:landingPage "https://www.legislation.gov.au/F2021L00312/asmade/2021-03-24/text/original/epub/OEBPS/document_1/document_1.html#_Toc65843542"^^xsd:anyURI ;
    dcat:theme legcons:Item .

F2021L00312:259 a legcons:Item,
        owl:Class,
        dcat:Resource ;
    rdfs:label "Item - I259 11 14  Amount of compensation"@en-AU ;
    dct:isPartOf F2021L00312:257 ;
    dct:isReferencedBy F2021L00312: ;
    rdfs:comment "11 14  Amount of compensation - Abrievated Graph Key: I259"@en-AU ;
    skos:definition "11 14  Amount of compensation"@en-AU ;
    skos:narrower F2021L00312:257 ;
    skos:prefLabel "Item I259"@en-AU ;
    dcat:accessURL <https://www.legislation.gov.au/F2021L00312/asmade/2021-03-24/text/original/epub/OEBPS/document_1/document_1.html#_Toc65843543> ;
    dcat:landingPage "https://www.legislation.gov.au/F2021L00312/asmade/2021-03-24/text/original/epub/OEBPS/document_1/document_1.html#_Toc65843543"^^xsd:anyURI ;
    dcat:theme legcons:Item .

F2021L00312:26 a legcons:Item,
        owl:Class,
        dcat:Resource ;
    rdfs:label "Item - I26 2 12  Variation of conditions of exemptionmatters to which Secretary must have regard"@en-AU ;
    dct:isPartOf F2021L00312:10 ;
    dct:isReferencedBy F2021L00312: ;
    rdfs:comment "2 12  Variation of conditions of exemptionmatters to which Secretary must have regard - Abrievated Graph Key: I26"@en-AU ;
    skos:definition "2 12  Variation of conditions of exemptionmatters to which Secretary must have regard"@en-AU ;
    skos:narrower F2021L00312:10 ;
    skos:prefLabel "Item I26"@en-AU ;
    dcat:accessURL <https://www.legislation.gov.au/F2021L00312/asmade/2021-03-24/text/original/epub/OEBPS/document_1/document_1.html#_Toc65843310> ;
    dcat:landingPage "https://www.legislation.gov.au/F2021L00312/asmade/2021-03-24/text/original/epub/OEBPS/document_1/document_1.html#_Toc65843310"^^xsd:anyURI ;
    dcat:theme legcons:Item .

F2021L00312:261 a legcons:Item,
        owl:Class,
        dcat:Resource ;
    rdfs:label "Item - I261 11 15  Circumstances in which relevant Commonwealth liability of a person is taken to have been paid"@en-AU ;
    dct:isPartOf F2021L00312:260 ;
    dct:isReferencedBy F2021L00312: ;
    rdfs:comment "11 15  Circumstances in which relevant Commonwealth liability of a person is taken to have been paid - Abrievated Graph Key: I261"@en-AU ;
    skos:definition "11 15  Circumstances in which relevant Commonwealth liability of a person is taken to have been paid"@en-AU ;
    skos:narrower F2021L00312:260 ;
    skos:prefLabel "Item I261"@en-AU ;
    dcat:accessURL <https://www.legislation.gov.au/F2021L00312/asmade/2021-03-24/text/original/epub/OEBPS/document_1/document_1.html#_Toc65843545> ;
    dcat:landingPage "https://www.legislation.gov.au/F2021L00312/asmade/2021-03-24/text/original/epub/OEBPS/document_1/document_1.html#_Toc65843545"^^xsd:anyURI ;
    dcat:theme legcons:Item .

F2021L00312:264 a legcons:Item,
        owl:Class,
        dcat:Resource ;
    rdfs:label "Item - I264 12 1  Definitions"@en-AU ;
    dct:isPartOf F2021L00312:263 ;
    dct:isReferencedBy F2021L00312: ;
    rdfs:comment "12 1  Definitions - Abrievated Graph Key: I264"@en-AU ;
    skos:definition "12 1  Definitions"@en-AU ;
    skos:narrower F2021L00312:263 ;
    skos:prefLabel "Item I264"@en-AU ;
    dcat:accessURL <https://www.legislation.gov.au/F2021L00312/asmade/2021-03-24/text/original/epub/OEBPS/document_1/document_1.html#_Toc65843548> ;
    dcat:landingPage "https://www.legislation.gov.au/F2021L00312/asmade/2021-03-24/text/original/epub/OEBPS/document_1/document_1.html#_Toc65843548"^^xsd:anyURI ;
    dcat:theme legcons:Item .

F2021L00312:266 a legcons:Item,
        owl:Class,
        dcat:Resource ;
    rdfs:label "Item - I266 12 2  Information and declarations given before commencement time"@en-AU ;
    dct:isPartOf F2021L00312:265 ;
    dct:isReferencedBy F2021L00312: ;
    rdfs:comment "12 2  Information and declarations given before commencement time - Abrievated Graph Key: I266"@en-AU ;
    skos:definition "12 2  Information and declarations given before commencement time"@en-AU ;
    skos:narrower F2021L00312:265 ;
    skos:prefLabel "Item I266"@en-AU ;
    dcat:accessURL <https://www.legislation.gov.au/F2021L00312/asmade/2021-03-24/text/original/epub/OEBPS/document_1/document_1.html#_Toc65843550> ;
    dcat:landingPage "https://www.legislation.gov.au/F2021L00312/asmade/2021-03-24/text/original/epub/OEBPS/document_1/document_1.html#_Toc65843550"^^xsd:anyURI ;
    dcat:theme legcons:Item .

F2021L00312:269 a legcons:Item,
        owl:Class,
        dcat:Resource ;
    rdfs:label "Item - I269 12 3  Request for translation not complied with before commencement time"@en-AU ;
    dct:isPartOf F2021L00312:268 ;
    dct:isReferencedBy F2021L00312: ;
    rdfs:comment "12 3  Request for translation not complied with before commencement time - Abrievated Graph Key: I269"@en-AU ;
    skos:definition "12 3  Request for translation not complied with before commencement time"@en-AU ;
    skos:narrower F2021L00312:268 ;
    skos:prefLabel "Item I269"@en-AU ;
    dcat:accessURL <https://www.legislation.gov.au/F2021L00312/asmade/2021-03-24/text/original/epub/OEBPS/document_1/document_1.html#_Toc65843553> ;
    dcat:landingPage "https://www.legislation.gov.au/F2021L00312/asmade/2021-03-24/text/original/epub/OEBPS/document_1/document_1.html#_Toc65843553"^^xsd:anyURI ;
    dcat:theme legcons:Item .

F2021L00312:27 a legcons:Part,
        owl:Class,
        dcat:Resource ;
    rdfs:label "Part - P27 Part 3 Government certificates"@en-AU ;
    dct:isPartOf F2021L00312:10 ;
    dct:isReferencedBy F2021L00312: ;
    rdfs:comment "Part 3 Government certificates - Abrievated Graph Key: P27"@en-AU ;
    skos:definition "Part 3 Government certificates"@en-AU ;
    skos:narrower F2021L00312:10 ;
    skos:prefLabel "Part P27"@en-AU ;
    dcat:accessURL <https://www.legislation.gov.au/F2021L00312/asmade/2021-03-24/text/original/epub/OEBPS/document_1/document_1.html#_Toc65843311> ;
    dcat:landingPage "https://www.legislation.gov.au/F2021L00312/asmade/2021-03-24/text/original/epub/OEBPS/document_1/document_1.html#_Toc65843311"^^xsd:anyURI ;
    dcat:theme legcons:Part .

F2021L00312:271 a legcons:Item,
        owl:Class,
        dcat:Resource ;
    rdfs:label "Item - I271 12 4  Person approved before commencement time to manufacture an official mark"@en-AU ;
    dct:isPartOf F2021L00312:270 ;
    dct:isReferencedBy F2021L00312: ;
    rdfs:comment "12 4  Person approved before commencement time to manufacture an official mark - Abrievated Graph Key: I271"@en-AU ;
    skos:definition "12 4  Person approved before commencement time to manufacture an official mark"@en-AU ;
    skos:narrower F2021L00312:270 ;
    skos:prefLabel "Item I271"@en-AU ;
    dcat:accessURL <https://www.legislation.gov.au/F2021L00312/asmade/2021-03-24/text/original/epub/OEBPS/document_1/document_1.html#_Toc65843555> ;
    dcat:landingPage "https://www.legislation.gov.au/F2021L00312/asmade/2021-03-24/text/original/epub/OEBPS/document_1/document_1.html#_Toc65843555"^^xsd:anyURI ;
    dcat:theme legcons:Item .

F2021L00312:272 a legcons:Item,
        owl:Class,
        dcat:Resource ;
    rdfs:label "Item - I272 12 5  Person approved before commencement time to possess an official mark"@en-AU ;
    dct:isPartOf F2021L00312:270 ;
    dct:isReferencedBy F2021L00312: ;
    rdfs:comment "12 5  Person approved before commencement time to possess an official mark - Abrievated Graph Key: I272"@en-AU ;
    skos:definition "12 5  Person approved before commencement time to possess an official mark"@en-AU ;
    skos:narrower F2021L00312:270 ;
    skos:prefLabel "Item I272"@en-AU ;
    dcat:accessURL <https://www.legislation.gov.au/F2021L00312/asmade/2021-03-24/text/original/epub/OEBPS/document_1/document_1.html#_Toc65843556> ;
    dcat:landingPage "https://www.legislation.gov.au/F2021L00312/asmade/2021-03-24/text/original/epub/OEBPS/document_1/document_1.html#_Toc65843556"^^xsd:anyURI ;
    dcat:theme legcons:Item .

F2021L00312:273 a legcons:Item,
        owl:Class,
        dcat:Resource ;
    rdfs:label "Item - I273 12 6  Person approved before commencement time to apply an official mark"@en-AU ;
    dct:isPartOf F2021L00312:270 ;
    dct:isReferencedBy F2021L00312: ;
    rdfs:comment "12 6  Person approved before commencement time to apply an official mark - Abrievated Graph Key: I273"@en-AU ;
    skos:definition "12 6  Person approved before commencement time to apply an official mark"@en-AU ;
    skos:narrower F2021L00312:270 ;
    skos:prefLabel "Item I273"@en-AU ;
    dcat:accessURL <https://www.legislation.gov.au/F2021L00312/asmade/2021-03-24/text/original/epub/OEBPS/document_1/document_1.html#_Toc65843557> ;
    dcat:landingPage "https://www.legislation.gov.au/F2021L00312/asmade/2021-03-24/text/original/epub/OEBPS/document_1/document_1.html#_Toc65843557"^^xsd:anyURI ;
    dcat:theme legcons:Item .

F2021L00312:275 a legcons:Item,
        owl:Class,
        dcat:Resource ;
    rdfs:label "Item - I275 12 7  Person approved before commencement time to manufacture an official marking device"@en-AU ;
    dct:isPartOf F2021L00312:274 ;
    dct:isReferencedBy F2021L00312: ;
    rdfs:comment "12 7  Person approved before commencement time to manufacture an official marking device - Abrievated Graph Key: I275"@en-AU ;
    skos:definition "12 7  Person approved before commencement time to manufacture an official marking device"@en-AU ;
    skos:narrower F2021L00312:274 ;
    skos:prefLabel "Item I275"@en-AU ;
    dcat:accessURL <https://www.legislation.gov.au/F2021L00312/asmade/2021-03-24/text/original/epub/OEBPS/document_1/document_1.html#_Toc65843559> ;
    dcat:landingPage "https://www.legislation.gov.au/F2021L00312/asmade/2021-03-24/text/original/epub/OEBPS/document_1/document_1.html#_Toc65843559"^^xsd:anyURI ;
    dcat:theme legcons:Item .

F2021L00312:276 a legcons:Item,
        owl:Class,
        dcat:Resource ;
    rdfs:label "Item - I276 12 8  Person approved before commencement time to possess an official marking device"@en-AU ;
    dct:isPartOf F2021L00312:274 ;
    dct:isReferencedBy F2021L00312: ;
    rdfs:comment "12 8  Person approved before commencement time to possess an official marking device - Abrievated Graph Key: I276"@en-AU ;
    skos:definition "12 8  Person approved before commencement time to possess an official marking device"@en-AU ;
    skos:narrower F2021L00312:274 ;
    skos:prefLabel "Item I276"@en-AU ;
    dcat:accessURL <https://www.legislation.gov.au/F2021L00312/asmade/2021-03-24/text/original/epub/OEBPS/document_1/document_1.html#_Toc65843560> ;
    dcat:landingPage "https://www.legislation.gov.au/F2021L00312/asmade/2021-03-24/text/original/epub/OEBPS/document_1/document_1.html#_Toc65843560"^^xsd:anyURI ;
    dcat:theme legcons:Item .

F2021L00312:279 a legcons:Item,
        owl:Class,
        dcat:Resource ;
    rdfs:label "Item - I279 12 9  Application for approval as auditor not decided or notice of decision not given before commencement time"@en-AU ;
    dct:isPartOf F2021L00312:278 ;
    dct:isReferencedBy F2021L00312: ;
    rdfs:comment "12 9  Application for approval as auditor not decided or notice of decision not given before commencement time - Abrievated Graph Key: I279"@en-AU ;
    skos:definition "12 9  Application for approval as auditor not decided or notice of decision not given before commencement time"@en-AU ;
    skos:narrower F2021L00312:278 ;
    skos:prefLabel "Item I279"@en-AU ;
    dcat:accessURL <https://www.legislation.gov.au/F2021L00312/asmade/2021-03-24/text/original/epub/OEBPS/document_1/document_1.html#_Toc65843563> ;
    dcat:landingPage "https://www.legislation.gov.au/F2021L00312/asmade/2021-03-24/text/original/epub/OEBPS/document_1/document_1.html#_Toc65843563"^^xsd:anyURI ;
    dcat:theme legcons:Item .

F2021L00312:28 a legcons:Item,
        owl:Class,
        dcat:Resource ;
    rdfs:label "Item - I28 2 13  When government certificate may be issued in relation to eggs or egg products"@en-AU ;
    dct:isPartOf F2021L00312:10 ;
    dct:isReferencedBy F2021L00312: ;
    rdfs:comment "2 13  When government certificate may be issued in relation to eggs or egg products - Abrievated Graph Key: I28"@en-AU ;
    skos:definition "2 13  When government certificate may be issued in relation to eggs or egg products"@en-AU ;
    skos:narrower F2021L00312:10 ;
    skos:prefLabel "Item I28"@en-AU ;
    dcat:accessURL <https://www.legislation.gov.au/F2021L00312/asmade/2021-03-24/text/original/epub/OEBPS/document_1/document_1.html#_Toc65843312> ;
    dcat:landingPage "https://www.legislation.gov.au/F2021L00312/asmade/2021-03-24/text/original/epub/OEBPS/document_1/document_1.html#_Toc65843312"^^xsd:anyURI ;
    dcat:theme legcons:Item .

F2021L00312:280 a legcons:Item,
        owl:Class,
        dcat:Resource ;
    rdfs:label "Item - I280 12 10  Request for further information not complied with before commencement time"@en-AU ;
    dct:isPartOf F2021L00312:278 ;
    dct:isReferencedBy F2021L00312: ;
    rdfs:comment "12 10  Request for further information not complied with before commencement time - Abrievated Graph Key: I280"@en-AU ;
    skos:definition "12 10  Request for further information not complied with before commencement time"@en-AU ;
    skos:narrower F2021L00312:278 ;
    skos:prefLabel "Item I280"@en-AU ;
    dcat:accessURL <https://www.legislation.gov.au/F2021L00312/asmade/2021-03-24/text/original/epub/OEBPS/document_1/document_1.html#_Toc65843564> ;
    dcat:landingPage "https://www.legislation.gov.au/F2021L00312/asmade/2021-03-24/text/original/epub/OEBPS/document_1/document_1.html#_Toc65843564"^^xsd:anyURI ;
    dcat:theme legcons:Item .

F2021L00312:281 a legcons:Item,
        owl:Class,
        dcat:Resource ;
    rdfs:label "Item - I281 12 11  Decision to revoke approval as auditor decided but notice not given before commencement time"@en-AU ;
    dct:isPartOf F2021L00312:278 ;
    dct:isReferencedBy F2021L00312: ;
    rdfs:comment "12 11  Decision to revoke approval as auditor decided but notice not given before commencement time - Abrievated Graph Key: I281"@en-AU ;
    skos:definition "12 11  Decision to revoke approval as auditor decided but notice not given before commencement time"@en-AU ;
    skos:narrower F2021L00312:278 ;
    skos:prefLabel "Item I281"@en-AU ;
    dcat:accessURL <https://www.legislation.gov.au/F2021L00312/asmade/2021-03-24/text/original/epub/OEBPS/document_1/document_1.html#_Toc65843565> ;
    dcat:landingPage "https://www.legislation.gov.au/F2021L00312/asmade/2021-03-24/text/original/epub/OEBPS/document_1/document_1.html#_Toc65843565"^^xsd:anyURI ;
    dcat:theme legcons:Item .

F2021L00312:283 a legcons:Item,
        owl:Class,
        dcat:Resource ;
    rdfs:label "Item - I283 12 12  Verification by authorised officer before commencement time"@en-AU ;
    dct:isPartOf F2021L00312:282 ;
    dct:isReferencedBy F2021L00312: ;
    rdfs:comment "12 12  Verification by authorised officer before commencement time - Abrievated Graph Key: I283"@en-AU ;
    skos:definition "12 12  Verification by authorised officer before commencement time"@en-AU ;
    skos:narrower F2021L00312:282 ;
    skos:prefLabel "Item I283"@en-AU ;
    dcat:accessURL <https://www.legislation.gov.au/F2021L00312/asmade/2021-03-24/text/original/epub/OEBPS/document_1/document_1.html#_Toc65843567> ;
    dcat:landingPage "https://www.legislation.gov.au/F2021L00312/asmade/2021-03-24/text/original/epub/OEBPS/document_1/document_1.html#_Toc65843567"^^xsd:anyURI ;
    dcat:theme legcons:Item .

F2021L00312:29 a legcons:Item,
        owl:Class,
        dcat:Resource ;
    rdfs:label "Item - I29 2 14  Matters stated in government certificatemanufacturing grade eggs or egg products"@en-AU ;
    dct:isPartOf F2021L00312:10 ;
    dct:isReferencedBy F2021L00312: ;
    rdfs:comment "2 14  Matters stated in government certificatemanufacturing grade eggs or egg products - Abrievated Graph Key: I29"@en-AU ;
    skos:definition "2 14  Matters stated in government certificatemanufacturing grade eggs or egg products"@en-AU ;
    skos:narrower F2021L00312:10 ;
    skos:prefLabel "Item I29"@en-AU ;
    dcat:accessURL <https://www.legislation.gov.au/F2021L00312/asmade/2021-03-24/text/original/epub/OEBPS/document_1/document_1.html#_Toc65843313> ;
    dcat:landingPage "https://www.legislation.gov.au/F2021L00312/asmade/2021-03-24/text/original/epub/OEBPS/document_1/document_1.html#_Toc65843313"^^xsd:anyURI ;
    dcat:theme legcons:Item .

F2021L00312:3 a legcons:Item,
        owl:Class,
        dcat:Resource ;
    rdfs:label "Item - I3 1 1  Name"@en-AU ;
    dct:isPartOf F2021L00312:1 ;
    dct:isReferencedBy F2021L00312: ;
    rdfs:comment "1 1  Name - Abrievated Graph Key: I3"@en-AU ;
    skos:definition "1 1  Name"@en-AU ;
    skos:narrower F2021L00312:1 ;
    skos:prefLabel "Item I3"@en-AU ;
    dcat:accessURL <https://www.legislation.gov.au/F2021L00312/asmade/2021-03-24/text/original/epub/OEBPS/document_1/document_1.html#_Toc65843287> ;
    dcat:landingPage "https://www.legislation.gov.au/F2021L00312/asmade/2021-03-24/text/original/epub/OEBPS/document_1/document_1.html#_Toc65843287"^^xsd:anyURI ;
    dcat:theme legcons:Item .

F2021L00312:30 a legcons:Item,
        owl:Class,
        dcat:Resource ;
    rdfs:label "Item - I30 2 15  Requirements before issue of government certificatecondition of eggs or egg products"@en-AU ;
    dct:isPartOf F2021L00312:10 ;
    dct:isReferencedBy F2021L00312: ;
    rdfs:comment "2 15  Requirements before issue of government certificatecondition of eggs or egg products - Abrievated Graph Key: I30"@en-AU ;
    skos:definition "2 15  Requirements before issue of government certificatecondition of eggs or egg products"@en-AU ;
    skos:narrower F2021L00312:10 ;
    skos:prefLabel "Item I30"@en-AU ;
    dcat:accessURL <https://www.legislation.gov.au/F2021L00312/asmade/2021-03-24/text/original/epub/OEBPS/document_1/document_1.html#_Toc65843314> ;
    dcat:landingPage "https://www.legislation.gov.au/F2021L00312/asmade/2021-03-24/text/original/epub/OEBPS/document_1/document_1.html#_Toc65843314"^^xsd:anyURI ;
    dcat:theme legcons:Item .

F2021L00312:31 a legcons:Item,
        owl:Class,
        dcat:Resource ;
    rdfs:label "Item - I31 2 16  Circumstances for refusing to issue government certificate"@en-AU ;
    dct:isPartOf F2021L00312:10 ;
    dct:isReferencedBy F2021L00312: ;
    rdfs:comment "2 16  Circumstances for refusing to issue government certificate - Abrievated Graph Key: I31"@en-AU ;
    skos:definition "2 16  Circumstances for refusing to issue government certificate"@en-AU ;
    skos:narrower F2021L00312:10 ;
    skos:prefLabel "Item I31"@en-AU ;
    dcat:accessURL <https://www.legislation.gov.au/F2021L00312/asmade/2021-03-24/text/original/epub/OEBPS/document_1/document_1.html#_Toc65843315> ;
    dcat:landingPage "https://www.legislation.gov.au/F2021L00312/asmade/2021-03-24/text/original/epub/OEBPS/document_1/document_1.html#_Toc65843315"^^xsd:anyURI ;
    dcat:theme legcons:Item .

F2021L00312:32 a legcons:Item,
        owl:Class,
        dcat:Resource ;
    rdfs:label "Item - I32 2 17  Changes that require holder of certificate to give additional or corrected information to issuing body"@en-AU ;
    dct:isPartOf F2021L00312:10 ;
    dct:isReferencedBy F2021L00312: ;
    rdfs:comment "2 17  Changes that require holder of certificate to give additional or corrected information to issuing body - Abrievated Graph Key: I32"@en-AU ;
    skos:definition "2 17  Changes that require holder of certificate to give additional or corrected information to issuing body"@en-AU ;
    skos:narrower F2021L00312:10 ;
    skos:prefLabel "Item I32"@en-AU ;
    dcat:accessURL <https://www.legislation.gov.au/F2021L00312/asmade/2021-03-24/text/original/epub/OEBPS/document_1/document_1.html#_Toc65843316> ;
    dcat:landingPage "https://www.legislation.gov.au/F2021L00312/asmade/2021-03-24/text/original/epub/OEBPS/document_1/document_1.html#_Toc65843316"^^xsd:anyURI ;
    dcat:theme legcons:Item .

F2021L00312:33 a legcons:Item,
        owl:Class,
        dcat:Resource ;
    rdfs:label "Item - I33 2 18  Return of government certificate"@en-AU ;
    dct:isPartOf F2021L00312:10 ;
    dct:isReferencedBy F2021L00312: ;
    rdfs:comment "2 18  Return of government certificate - Abrievated Graph Key: I33"@en-AU ;
    skos:definition "2 18  Return of government certificate"@en-AU ;
    skos:narrower F2021L00312:10 ;
    skos:prefLabel "Item I33"@en-AU ;
    dcat:accessURL <https://www.legislation.gov.au/F2021L00312/asmade/2021-03-24/text/original/epub/OEBPS/document_1/document_1.html#_Toc65843317> ;
    dcat:landingPage "https://www.legislation.gov.au/F2021L00312/asmade/2021-03-24/text/original/epub/OEBPS/document_1/document_1.html#_Toc65843317"^^xsd:anyURI ;
    dcat:theme legcons:Item .

F2021L00312:37 a legcons:Item,
        owl:Class,
        dcat:Resource ;
    rdfs:label "Item - I37 4 1  Purpose of this Division"@en-AU ;
    dct:isPartOf F2021L00312:36 ;
    dct:isReferencedBy F2021L00312: ;
    rdfs:comment "4 1  Purpose of this Division - Abrievated Graph Key: I37"@en-AU ;
    skos:definition "4 1  Purpose of this Division"@en-AU ;
    skos:narrower F2021L00312:36 ;
    skos:prefLabel "Item I37"@en-AU ;
    dcat:accessURL <https://www.legislation.gov.au/F2021L00312/asmade/2021-03-24/text/original/epub/OEBPS/document_1/document_1.html#_Toc65843321> ;
    dcat:landingPage "https://www.legislation.gov.au/F2021L00312/asmade/2021-03-24/text/original/epub/OEBPS/document_1/document_1.html#_Toc65843321"^^xsd:anyURI ;
    dcat:theme legcons:Item .

F2021L00312:38 a legcons:Item,
        owl:Class,
        dcat:Resource ;
    rdfs:label "Item - I38 4 2  Equipment facilities and essential servicesgeneral"@en-AU ;
    dct:isPartOf F2021L00312:36 ;
    dct:isReferencedBy F2021L00312: ;
    rdfs:comment "4 2  Equipment facilities and essential servicesgeneral - Abrievated Graph Key: I38"@en-AU ;
    skos:definition "4 2  Equipment facilities and essential servicesgeneral"@en-AU ;
    skos:narrower F2021L00312:36 ;
    skos:prefLabel "Item I38"@en-AU ;
    dcat:accessURL <https://www.legislation.gov.au/F2021L00312/asmade/2021-03-24/text/original/epub/OEBPS/document_1/document_1.html#_Toc65843322> ;
    dcat:landingPage "https://www.legislation.gov.au/F2021L00312/asmade/2021-03-24/text/original/epub/OEBPS/document_1/document_1.html#_Toc65843322"^^xsd:anyURI ;
    dcat:theme legcons:Item .

F2021L00312:39 a legcons:Item,
        owl:Class,
        dcat:Resource ;
    rdfs:label "Item - I39 4 3  Measuring devices"@en-AU ;
    dct:isPartOf F2021L00312:36 ;
    dct:isReferencedBy F2021L00312: ;
    rdfs:comment "4 3  Measuring devices - Abrievated Graph Key: I39"@en-AU ;
    skos:definition "4 3  Measuring devices"@en-AU ;
    skos:narrower F2021L00312:36 ;
    skos:prefLabel "Item I39"@en-AU ;
    dcat:accessURL <https://www.legislation.gov.au/F2021L00312/asmade/2021-03-24/text/original/epub/OEBPS/document_1/document_1.html#_Toc65843323> ;
    dcat:landingPage "https://www.legislation.gov.au/F2021L00312/asmade/2021-03-24/text/original/epub/OEBPS/document_1/document_1.html#_Toc65843323"^^xsd:anyURI ;
    dcat:theme legcons:Item .

F2021L00312:4 a legcons:Item,
        owl:Class,
        dcat:Resource ;
    rdfs:label "Item - I4 1 2  Commencement"@en-AU ;
    dct:isPartOf F2021L00312:1 ;
    dct:isReferencedBy F2021L00312: ;
    rdfs:comment "1 2  Commencement - Abrievated Graph Key: I4"@en-AU ;
    skos:definition "1 2  Commencement"@en-AU ;
    skos:narrower F2021L00312:1 ;
    skos:prefLabel "Item I4"@en-AU ;
    dcat:accessURL <https://www.legislation.gov.au/F2021L00312/asmade/2021-03-24/text/original/epub/OEBPS/document_1/document_1.html#_Toc65843288> ;
    dcat:landingPage "https://www.legislation.gov.au/F2021L00312/asmade/2021-03-24/text/original/epub/OEBPS/document_1/document_1.html#_Toc65843288"^^xsd:anyURI ;
    dcat:theme legcons:Item .

F2021L00312:40 a legcons:Item,
        owl:Class,
        dcat:Resource ;
    rdfs:label "Item - I40 4 4  Establishment including construction"@en-AU ;
    dct:isPartOf F2021L00312:36 ;
    dct:isReferencedBy F2021L00312: ;
    rdfs:comment "4 4  Establishment including construction - Abrievated Graph Key: I40"@en-AU ;
    skos:definition "4 4  Establishment including construction"@en-AU ;
    skos:narrower F2021L00312:36 ;
    skos:prefLabel "Item I40"@en-AU ;
    dcat:accessURL <https://www.legislation.gov.au/F2021L00312/asmade/2021-03-24/text/original/epub/OEBPS/document_1/document_1.html#_Toc65843324> ;
    dcat:landingPage "https://www.legislation.gov.au/F2021L00312/asmade/2021-03-24/text/original/epub/OEBPS/document_1/document_1.html#_Toc65843324"^^xsd:anyURI ;
    dcat:theme legcons:Item .

F2021L00312:41 a legcons:Item,
        owl:Class,
        dcat:Resource ;
    rdfs:label "Item - I41 4 5  Fixtures fittings and equipment"@en-AU ;
    dct:isPartOf F2021L00312:36 ;
    dct:isReferencedBy F2021L00312: ;
    rdfs:comment "4 5  Fixtures fittings and equipment - Abrievated Graph Key: I41"@en-AU ;
    skos:definition "4 5  Fixtures fittings and equipment"@en-AU ;
    skos:narrower F2021L00312:36 ;
    skos:prefLabel "Item I41"@en-AU ;
    dcat:accessURL <https://www.legislation.gov.au/F2021L00312/asmade/2021-03-24/text/original/epub/OEBPS/document_1/document_1.html#_Toc65843325> ;
    dcat:landingPage "https://www.legislation.gov.au/F2021L00312/asmade/2021-03-24/text/original/epub/OEBPS/document_1/document_1.html#_Toc65843325"^^xsd:anyURI ;
    dcat:theme legcons:Item .

F2021L00312:42 a legcons:Item,
        owl:Class,
        dcat:Resource ;
    rdfs:label "Item - I42 4 6  Storage facilities for items other than eggs or egg products"@en-AU ;
    dct:isPartOf F2021L00312:36 ;
    dct:isReferencedBy F2021L00312: ;
    rdfs:comment "4 6  Storage facilities for items other than eggs or egg products - Abrievated Graph Key: I42"@en-AU ;
    skos:definition "4 6  Storage facilities for items other than eggs or egg products"@en-AU ;
    skos:narrower F2021L00312:36 ;
    skos:prefLabel "Item I42"@en-AU ;
    dcat:accessURL <https://www.legislation.gov.au/F2021L00312/asmade/2021-03-24/text/original/epub/OEBPS/document_1/document_1.html#_Toc65843326> ;
    dcat:landingPage "https://www.legislation.gov.au/F2021L00312/asmade/2021-03-24/text/original/epub/OEBPS/document_1/document_1.html#_Toc65843326"^^xsd:anyURI ;
    dcat:theme legcons:Item .

F2021L00312:43 a legcons:Item,
        owl:Class,
        dcat:Resource ;
    rdfs:label "Item - I43 4 7  Cleaning and sanitising facilities"@en-AU ;
    dct:isPartOf F2021L00312:36 ;
    dct:isReferencedBy F2021L00312: ;
    rdfs:comment "4 7  Cleaning and sanitising facilities - Abrievated Graph Key: I43"@en-AU ;
    skos:definition "4 7  Cleaning and sanitising facilities"@en-AU ;
    skos:narrower F2021L00312:36 ;
    skos:prefLabel "Item I43"@en-AU ;
    dcat:accessURL <https://www.legislation.gov.au/F2021L00312/asmade/2021-03-24/text/original/epub/OEBPS/document_1/document_1.html#_Toc65843327> ;
    dcat:landingPage "https://www.legislation.gov.au/F2021L00312/asmade/2021-03-24/text/original/epub/OEBPS/document_1/document_1.html#_Toc65843327"^^xsd:anyURI ;
    dcat:theme legcons:Item .

F2021L00312:44 a legcons:Item,
        owl:Class,
        dcat:Resource ;
    rdfs:label "Item - I44 4 8  Amenities"@en-AU ;
    dct:isPartOf F2021L00312:36 ;
    dct:isReferencedBy F2021L00312: ;
    rdfs:comment "4 8  Amenities - Abrievated Graph Key: I44"@en-AU ;
    skos:definition "4 8  Amenities"@en-AU ;
    skos:narrower F2021L00312:36 ;
    skos:prefLabel "Item I44"@en-AU ;
    dcat:accessURL <https://www.legislation.gov.au/F2021L00312/asmade/2021-03-24/text/original/epub/OEBPS/document_1/document_1.html#_Toc65843328> ;
    dcat:landingPage "https://www.legislation.gov.au/F2021L00312/asmade/2021-03-24/text/original/epub/OEBPS/document_1/document_1.html#_Toc65843328"^^xsd:anyURI ;
    dcat:theme legcons:Item .

F2021L00312:45 a legcons:Item,
        owl:Class,
        dcat:Resource ;
    rdfs:label "Item - I45 4 9  Essential services"@en-AU ;
    dct:isPartOf F2021L00312:36 ;
    dct:isReferencedBy F2021L00312: ;
    rdfs:comment "4 9  Essential services - Abrievated Graph Key: I45"@en-AU ;
    skos:definition "4 9  Essential services"@en-AU ;
    skos:narrower F2021L00312:36 ;
    skos:prefLabel "Item I45"@en-AU ;
    dcat:accessURL <https://www.legislation.gov.au/F2021L00312/asmade/2021-03-24/text/original/epub/OEBPS/document_1/document_1.html#_Toc65843329> ;
    dcat:landingPage "https://www.legislation.gov.au/F2021L00312/asmade/2021-03-24/text/original/epub/OEBPS/document_1/document_1.html#_Toc65843329"^^xsd:anyURI ;
    dcat:theme legcons:Item .

F2021L00312:47 a legcons:Item,
        owl:Class,
        dcat:Resource ;
    rdfs:label "Item - I47 4 10  Purpose of this Division"@en-AU ;
    dct:isPartOf F2021L00312:46 ;
    dct:isReferencedBy F2021L00312: ;
    rdfs:comment "4 10  Purpose of this Division - Abrievated Graph Key: I47"@en-AU ;
    skos:definition "4 10  Purpose of this Division"@en-AU ;
    skos:narrower F2021L00312:46 ;
    skos:prefLabel "Item I47"@en-AU ;
    dcat:accessURL <https://www.legislation.gov.au/F2021L00312/asmade/2021-03-24/text/original/epub/OEBPS/document_1/document_1.html#_Toc65843331> ;
    dcat:landingPage "https://www.legislation.gov.au/F2021L00312/asmade/2021-03-24/text/original/epub/OEBPS/document_1/document_1.html#_Toc65843331"^^xsd:anyURI ;
    dcat:theme legcons:Item .

F2021L00312:48 a legcons:Item,
        owl:Class,
        dcat:Resource ;
    rdfs:label "Item - I48 4 11  Operations must be carried out in a way that will ensure requirements of the Act are met"@en-AU ;
    dct:isPartOf F2021L00312:46 ;
    dct:isReferencedBy F2021L00312: ;
    rdfs:comment "4 11  Operations must be carried out in a way that will ensure requirements of the Act are met - Abrievated Graph Key: I48"@en-AU ;
    skos:definition "4 11  Operations must be carried out in a way that will ensure requirements of the Act are met"@en-AU ;
    skos:narrower F2021L00312:46 ;
    skos:prefLabel "Item I48"@en-AU ;
    dcat:accessURL <https://www.legislation.gov.au/F2021L00312/asmade/2021-03-24/text/original/epub/OEBPS/document_1/document_1.html#_Toc65843332> ;
    dcat:landingPage "https://www.legislation.gov.au/F2021L00312/asmade/2021-03-24/text/original/epub/OEBPS/document_1/document_1.html#_Toc65843332"^^xsd:anyURI ;
    dcat:theme legcons:Item .

F2021L00312:5 a legcons:Item,
        owl:Class,
        dcat:Resource ;
    rdfs:label "Item - I5 1 3  Authority"@en-AU ;
    dct:isPartOf F2021L00312:1 ;
    dct:isReferencedBy F2021L00312: ;
    rdfs:comment "1 3  Authority - Abrievated Graph Key: I5"@en-AU ;
    skos:definition "1 3  Authority"@en-AU ;
    skos:narrower F2021L00312:1 ;
    skos:prefLabel "Item I5"@en-AU ;
    dcat:accessURL <https://www.legislation.gov.au/F2021L00312/asmade/2021-03-24/text/original/epub/OEBPS/document_1/document_1.html#_Toc65843289> ;
    dcat:landingPage "https://www.legislation.gov.au/F2021L00312/asmade/2021-03-24/text/original/epub/OEBPS/document_1/document_1.html#_Toc65843289"^^xsd:anyURI ;
    dcat:theme legcons:Item .

F2021L00312:50 a legcons:Item,
        owl:Class,
        dcat:Resource ;
    rdfs:label "Item - I50 4 12  Purpose of this Part"@en-AU ;
    dct:isPartOf F2021L00312:49 ;
    dct:isReferencedBy F2021L00312: ;
    rdfs:comment "4 12  Purpose of this Part - Abrievated Graph Key: I50"@en-AU ;
    skos:definition "4 12  Purpose of this Part"@en-AU ;
    skos:narrower F2021L00312:49 ;
    skos:prefLabel "Item I50"@en-AU ;
    dcat:accessURL <https://www.legislation.gov.au/F2021L00312/asmade/2021-03-24/text/original/epub/OEBPS/document_1/document_1.html#_Toc65843334> ;
    dcat:landingPage "https://www.legislation.gov.au/F2021L00312/asmade/2021-03-24/text/original/epub/OEBPS/document_1/document_1.html#_Toc65843334"^^xsd:anyURI ;
    dcat:theme legcons:Item .

F2021L00312:51 a legcons:Item,
        owl:Class,
        dcat:Resource ;
    rdfs:label "Item - I51 4 13  Requirements for registration continue to be met"@en-AU ;
    dct:isPartOf F2021L00312:49 ;
    dct:isReferencedBy F2021L00312: ;
    rdfs:comment "4 13  Requirements for registration continue to be met - Abrievated Graph Key: I51"@en-AU ;
    skos:definition "4 13  Requirements for registration continue to be met"@en-AU ;
    skos:narrower F2021L00312:49 ;
    skos:prefLabel "Item I51"@en-AU ;
    dcat:accessURL <https://www.legislation.gov.au/F2021L00312/asmade/2021-03-24/text/original/epub/OEBPS/document_1/document_1.html#_Toc65843335> ;
    dcat:landingPage "https://www.legislation.gov.au/F2021L00312/asmade/2021-03-24/text/original/epub/OEBPS/document_1/document_1.html#_Toc65843335"^^xsd:anyURI ;
    dcat:theme legcons:Item .

F2021L00312:52 a legcons:Item,
        owl:Class,
        dcat:Resource ;
    rdfs:label "Item - I52 4 14  Other operational hygiene requirements"@en-AU ;
    dct:isPartOf F2021L00312:49 ;
    dct:isReferencedBy F2021L00312: ;
    rdfs:comment "4 14  Other operational hygiene requirements - Abrievated Graph Key: I52"@en-AU ;
    skos:definition "4 14  Other operational hygiene requirements"@en-AU ;
    skos:narrower F2021L00312:49 ;
    skos:prefLabel "Item I52"@en-AU ;
    dcat:accessURL <https://www.legislation.gov.au/F2021L00312/asmade/2021-03-24/text/original/epub/OEBPS/document_1/document_1.html#_Toc65843336> ;
    dcat:landingPage "https://www.legislation.gov.au/F2021L00312/asmade/2021-03-24/text/original/epub/OEBPS/document_1/document_1.html#_Toc65843336"^^xsd:anyURI ;
    dcat:theme legcons:Item .

F2021L00312:54 a legcons:Item,
        owl:Class,
        dcat:Resource ;
    rdfs:label "Item - I54 4 15  Period within which application to renew registration must be made"@en-AU ;
    dct:isPartOf F2021L00312:53 ;
    dct:isReferencedBy F2021L00312: ;
    rdfs:comment "4 15  Period within which application to renew registration must be made - Abrievated Graph Key: I54"@en-AU ;
    skos:definition "4 15  Period within which application to renew registration must be made"@en-AU ;
    skos:narrower F2021L00312:53 ;
    skos:prefLabel "Item I54"@en-AU ;
    dcat:accessURL <https://www.legislation.gov.au/F2021L00312/asmade/2021-03-24/text/original/epub/OEBPS/document_1/document_1.html#_Toc65843338> ;
    dcat:landingPage "https://www.legislation.gov.au/F2021L00312/asmade/2021-03-24/text/original/epub/OEBPS/document_1/document_1.html#_Toc65843338"^^xsd:anyURI ;
    dcat:theme legcons:Item .

F2021L00312:55 a legcons:Item,
        owl:Class,
        dcat:Resource ;
    rdfs:label "Item - I55 4 16  Requirements for renewal of registration"@en-AU ;
    dct:isPartOf F2021L00312:53 ;
    dct:isReferencedBy F2021L00312: ;
    rdfs:comment "4 16  Requirements for renewal of registration - Abrievated Graph Key: I55"@en-AU ;
    skos:definition "4 16  Requirements for renewal of registration"@en-AU ;
    skos:narrower F2021L00312:53 ;
    skos:prefLabel "Item I55"@en-AU ;
    dcat:accessURL <https://www.legislation.gov.au/F2021L00312/asmade/2021-03-24/text/original/epub/OEBPS/document_1/document_1.html#_Toc65843339> ;
    dcat:landingPage "https://www.legislation.gov.au/F2021L00312/asmade/2021-03-24/text/original/epub/OEBPS/document_1/document_1.html#_Toc65843339"^^xsd:anyURI ;
    dcat:theme legcons:Item .

F2021L00312:57 a legcons:Item,
        owl:Class,
        dcat:Resource ;
    rdfs:label "Item - I57 4 17  Request by occupier for suspension"@en-AU ;
    dct:isPartOf F2021L00312:56 ;
    dct:isReferencedBy F2021L00312: ;
    rdfs:comment "4 17  Request by occupier for suspension - Abrievated Graph Key: I57"@en-AU ;
    skos:definition "4 17  Request by occupier for suspension"@en-AU ;
    skos:narrower F2021L00312:56 ;
    skos:prefLabel "Item I57"@en-AU ;
    dcat:accessURL <https://www.legislation.gov.au/F2021L00312/asmade/2021-03-24/text/original/epub/OEBPS/document_1/document_1.html#_Toc65843341> ;
    dcat:landingPage "https://www.legislation.gov.au/F2021L00312/asmade/2021-03-24/text/original/epub/OEBPS/document_1/document_1.html#_Toc65843341"^^xsd:anyURI ;
    dcat:theme legcons:Item .

F2021L00312:58 a legcons:Item,
        owl:Class,
        dcat:Resource ;
    rdfs:label "Item - I58 4 18  Other grounds for suspension"@en-AU ;
    dct:isPartOf F2021L00312:56 ;
    dct:isReferencedBy F2021L00312: ;
    rdfs:comment "4 18  Other grounds for suspension - Abrievated Graph Key: I58"@en-AU ;
    skos:definition "4 18  Other grounds for suspension"@en-AU ;
    skos:narrower F2021L00312:56 ;
    skos:prefLabel "Item I58"@en-AU ;
    dcat:accessURL <https://www.legislation.gov.au/F2021L00312/asmade/2021-03-24/text/original/epub/OEBPS/document_1/document_1.html#_Toc65843342> ;
    dcat:landingPage "https://www.legislation.gov.au/F2021L00312/asmade/2021-03-24/text/original/epub/OEBPS/document_1/document_1.html#_Toc65843342"^^xsd:anyURI ;
    dcat:theme legcons:Item .

F2021L00312:6 a legcons:Item,
        owl:Class,
        dcat:Resource ;
    rdfs:label "Item - I6 1 4  Simplified outline of this instrument"@en-AU ;
    dct:isPartOf F2021L00312:1 ;
    dct:isReferencedBy F2021L00312: ;
    rdfs:comment "1 4  Simplified outline of this instrument - Abrievated Graph Key: I6"@en-AU ;
    skos:definition "1 4  Simplified outline of this instrument"@en-AU ;
    skos:narrower F2021L00312:1 ;
    skos:prefLabel "Item I6"@en-AU ;
    dcat:accessURL <https://www.legislation.gov.au/F2021L00312/asmade/2021-03-24/text/original/epub/OEBPS/document_1/document_1.html#_Toc65843290> ;
    dcat:landingPage "https://www.legislation.gov.au/F2021L00312/asmade/2021-03-24/text/original/epub/OEBPS/document_1/document_1.html#_Toc65843290"^^xsd:anyURI ;
    dcat:theme legcons:Item .

F2021L00312:60 a legcons:Item,
        owl:Class,
        dcat:Resource ;
    rdfs:label "Item - I60 4 19  Application of this Part"@en-AU ;
    dct:isPartOf F2021L00312:59 ;
    dct:isReferencedBy F2021L00312: ;
    rdfs:comment "4 19  Application of this Part - Abrievated Graph Key: I60"@en-AU ;
    skos:definition "4 19  Application of this Part"@en-AU ;
    skos:narrower F2021L00312:59 ;
    skos:prefLabel "Item I60"@en-AU ;
    dcat:accessURL <https://www.legislation.gov.au/F2021L00312/asmade/2021-03-24/text/original/epub/OEBPS/document_1/document_1.html#_Toc65843344> ;
    dcat:landingPage "https://www.legislation.gov.au/F2021L00312/asmade/2021-03-24/text/original/epub/OEBPS/document_1/document_1.html#_Toc65843344"^^xsd:anyURI ;
    dcat:theme legcons:Item .

F2021L00312:61 a legcons:Item,
        owl:Class,
        dcat:Resource ;
    rdfs:label "Item - I61 4 20  Initial consideration period"@en-AU ;
    dct:isPartOf F2021L00312:59 ;
    dct:isReferencedBy F2021L00312: ;
    rdfs:comment "4 20  Initial consideration period - Abrievated Graph Key: I61"@en-AU ;
    skos:definition "4 20  Initial consideration period"@en-AU ;
    skos:narrower F2021L00312:59 ;
    skos:prefLabel "Item I61"@en-AU ;
    dcat:accessURL <https://www.legislation.gov.au/F2021L00312/asmade/2021-03-24/text/original/epub/OEBPS/document_1/document_1.html#_Toc65843345> ;
    dcat:landingPage "https://www.legislation.gov.au/F2021L00312/asmade/2021-03-24/text/original/epub/OEBPS/document_1/document_1.html#_Toc65843345"^^xsd:anyURI ;
    dcat:theme legcons:Item .

F2021L00312:62 a legcons:Item,
        owl:Class,
        dcat:Resource ;
    rdfs:label "Item - I62 4 21  Period within which request relating to application must be complied with"@en-AU ;
    dct:isPartOf F2021L00312:59 ;
    dct:isReferencedBy F2021L00312: ;
    rdfs:comment "4 21  Period within which request relating to application must be complied with - Abrievated Graph Key: I62"@en-AU ;
    skos:definition "4 21  Period within which request relating to application must be complied with"@en-AU ;
    skos:narrower F2021L00312:59 ;
    skos:prefLabel "Item I62"@en-AU ;
    dcat:accessURL <https://www.legislation.gov.au/F2021L00312/asmade/2021-03-24/text/original/epub/OEBPS/document_1/document_1.html#_Toc65843346> ;
    dcat:landingPage "https://www.legislation.gov.au/F2021L00312/asmade/2021-03-24/text/original/epub/OEBPS/document_1/document_1.html#_Toc65843346"^^xsd:anyURI ;
    dcat:theme legcons:Item .

F2021L00312:65 a legcons:Item,
        owl:Class,
        dcat:Resource ;
    rdfs:label "Item - I65 5 1  Purpose of this Part"@en-AU ;
    dct:isPartOf F2021L00312:64 ;
    dct:isReferencedBy F2021L00312: ;
    rdfs:comment "5 1  Purpose of this Part - Abrievated Graph Key: I65"@en-AU ;
    skos:definition "5 1  Purpose of this Part"@en-AU ;
    skos:narrower F2021L00312:64 ;
    skos:prefLabel "Item I65"@en-AU ;
    dcat:accessURL <https://www.legislation.gov.au/F2021L00312/asmade/2021-03-24/text/original/epub/OEBPS/document_1/document_1.html#_Toc65843349> ;
    dcat:landingPage "https://www.legislation.gov.au/F2021L00312/asmade/2021-03-24/text/original/epub/OEBPS/document_1/document_1.html#_Toc65843349"^^xsd:anyURI ;
    dcat:theme legcons:Item .

F2021L00312:66 a legcons:Item,
        owl:Class,
        dcat:Resource ;
    rdfs:label "Item - I66 5 2  Proposed arrangement for operations to prepare prescribed eggs or egg products"@en-AU ;
    dct:isPartOf F2021L00312:64 ;
    dct:isReferencedBy F2021L00312: ;
    rdfs:comment "5 2  Proposed arrangement for operations to prepare prescribed eggs or egg products - Abrievated Graph Key: I66"@en-AU ;
    skos:definition "5 2  Proposed arrangement for operations to prepare prescribed eggs or egg products"@en-AU ;
    skos:narrower F2021L00312:64 ;
    skos:prefLabel "Item I66"@en-AU ;
    dcat:accessURL <https://www.legislation.gov.au/F2021L00312/asmade/2021-03-24/text/original/epub/OEBPS/document_1/document_1.html#_Toc65843350> ;
    dcat:landingPage "https://www.legislation.gov.au/F2021L00312/asmade/2021-03-24/text/original/epub/OEBPS/document_1/document_1.html#_Toc65843350"^^xsd:anyURI ;
    dcat:theme legcons:Item .

F2021L00312:67 a legcons:Item,
        owl:Class,
        dcat:Resource ;
    rdfs:label "Item - I67 5 3  Equipment"@en-AU ;
    dct:isPartOf F2021L00312:64 ;
    dct:isReferencedBy F2021L00312: ;
    rdfs:comment "5 3  Equipment - Abrievated Graph Key: I67"@en-AU ;
    skos:definition "5 3  Equipment"@en-AU ;
    skos:narrower F2021L00312:64 ;
    skos:prefLabel "Item I67"@en-AU ;
    dcat:accessURL <https://www.legislation.gov.au/F2021L00312/asmade/2021-03-24/text/original/epub/OEBPS/document_1/document_1.html#_Toc65843351> ;
    dcat:landingPage "https://www.legislation.gov.au/F2021L00312/asmade/2021-03-24/text/original/epub/OEBPS/document_1/document_1.html#_Toc65843351"^^xsd:anyURI ;
    dcat:theme legcons:Item .

F2021L00312:68 a legcons:Item,
        owl:Class,
        dcat:Resource ;
    rdfs:label "Item - I68 5 4  Operational hygiene"@en-AU ;
    dct:isPartOf F2021L00312:64 ;
    dct:isReferencedBy F2021L00312: ;
    rdfs:comment "5 4  Operational hygiene - Abrievated Graph Key: I68"@en-AU ;
    skos:definition "5 4  Operational hygiene"@en-AU ;
    skos:narrower F2021L00312:64 ;
    skos:prefLabel "Item I68"@en-AU ;
    dcat:accessURL <https://www.legislation.gov.au/F2021L00312/asmade/2021-03-24/text/original/epub/OEBPS/document_1/document_1.html#_Toc65843352> ;
    dcat:landingPage "https://www.legislation.gov.au/F2021L00312/asmade/2021-03-24/text/original/epub/OEBPS/document_1/document_1.html#_Toc65843352"^^xsd:anyURI ;
    dcat:theme legcons:Item .

F2021L00312:69 a legcons:Item,
        owl:Class,
        dcat:Resource ;
    rdfs:label "Item - I69 5 5  Identification traceability and integrity"@en-AU ;
    dct:isPartOf F2021L00312:64 ;
    dct:isReferencedBy F2021L00312: ;
    rdfs:comment "5 5  Identification traceability and integrity - Abrievated Graph Key: I69"@en-AU ;
    skos:definition "5 5  Identification traceability and integrity"@en-AU ;
    skos:narrower F2021L00312:64 ;
    skos:prefLabel "Item I69"@en-AU ;
    dcat:accessURL <https://www.legislation.gov.au/F2021L00312/asmade/2021-03-24/text/original/epub/OEBPS/document_1/document_1.html#_Toc65843353> ;
    dcat:landingPage "https://www.legislation.gov.au/F2021L00312/asmade/2021-03-24/text/original/epub/OEBPS/document_1/document_1.html#_Toc65843353"^^xsd:anyURI ;
    dcat:theme legcons:Item .

F2021L00312:7 a legcons:Part,
        owl:Class,
        dcat:Resource ;
    rdfs:label "Part - P7 Part 2 Interpretation"@en-AU ;
    dct:isPartOf F2021L00312:1 ;
    dct:isReferencedBy F2021L00312: ;
    rdfs:comment "Part 2 Interpretation - Abrievated Graph Key: P7"@en-AU ;
    skos:definition "Part 2 Interpretation"@en-AU ;
    skos:narrower F2021L00312:1 ;
    skos:prefLabel "Part P7"@en-AU ;
    dcat:accessURL <https://www.legislation.gov.au/F2021L00312/asmade/2021-03-24/text/original/epub/OEBPS/document_1/document_1.html#_Toc65843291> ;
    dcat:landingPage "https://www.legislation.gov.au/F2021L00312/asmade/2021-03-24/text/original/epub/OEBPS/document_1/document_1.html#_Toc65843291"^^xsd:anyURI ;
    dcat:theme legcons:Part .

F2021L00312:72 a legcons:Item,
        owl:Class,
        dcat:Resource ;
    rdfs:label "Item - I72 5 6  Purpose of this Part"@en-AU ;
    dct:isPartOf F2021L00312:71 ;
    dct:isReferencedBy F2021L00312: ;
    rdfs:comment "5 6  Purpose of this Part - Abrievated Graph Key: I72"@en-AU ;
    skos:definition "5 6  Purpose of this Part"@en-AU ;
    skos:narrower F2021L00312:71 ;
    skos:prefLabel "Item I72"@en-AU ;
    dcat:accessURL <https://www.legislation.gov.au/F2021L00312/asmade/2021-03-24/text/original/epub/OEBPS/document_1/document_1.html#_Toc65843356> ;
    dcat:landingPage "https://www.legislation.gov.au/F2021L00312/asmade/2021-03-24/text/original/epub/OEBPS/document_1/document_1.html#_Toc65843356"^^xsd:anyURI ;
    dcat:theme legcons:Item .

F2021L00312:74 a legcons:Item,
        owl:Class,
        dcat:Resource ;
    rdfs:label "Item - I74 5 7  Importing country requirements must be met"@en-AU ;
    dct:isPartOf F2021L00312:73 ;
    dct:isReferencedBy F2021L00312: ;
    rdfs:comment "5 7  Importing country requirements must be met - Abrievated Graph Key: I74"@en-AU ;
    skos:definition "5 7  Importing country requirements must be met"@en-AU ;
    skos:narrower F2021L00312:73 ;
    skos:prefLabel "Item I74"@en-AU ;
    dcat:accessURL <https://www.legislation.gov.au/F2021L00312/asmade/2021-03-24/text/original/epub/OEBPS/document_1/document_1.html#_Toc65843358> ;
    dcat:landingPage "https://www.legislation.gov.au/F2021L00312/asmade/2021-03-24/text/original/epub/OEBPS/document_1/document_1.html#_Toc65843358"^^xsd:anyURI ;
    dcat:theme legcons:Item .

F2021L00312:76 a legcons:Item,
        owl:Class,
        dcat:Resource ;
    rdfs:label "Item - I76 5 8  Purpose of this Division"@en-AU ;
    dct:isPartOf F2021L00312:75 ;
    dct:isReferencedBy F2021L00312: ;
    rdfs:comment "5 8  Purpose of this Division - Abrievated Graph Key: I76"@en-AU ;
    skos:definition "5 8  Purpose of this Division"@en-AU ;
    skos:narrower F2021L00312:75 ;
    skos:prefLabel "Item I76"@en-AU ;
    dcat:accessURL <https://www.legislation.gov.au/F2021L00312/asmade/2021-03-24/text/original/epub/OEBPS/document_1/document_1.html#_Toc65843360> ;
    dcat:landingPage "https://www.legislation.gov.au/F2021L00312/asmade/2021-03-24/text/original/epub/OEBPS/document_1/document_1.html#_Toc65843360"^^xsd:anyURI ;
    dcat:theme legcons:Item .

F2021L00312:77 a legcons:Item,
        owl:Class,
        dcat:Resource ;
    rdfs:label "Item - I77 5 9  Hygiene controlestablishment and its equipment"@en-AU ;
    dct:isPartOf F2021L00312:75 ;
    dct:isReferencedBy F2021L00312: ;
    rdfs:comment "5 9  Hygiene controlestablishment and its equipment - Abrievated Graph Key: I77"@en-AU ;
    skos:definition "5 9  Hygiene controlestablishment and its equipment"@en-AU ;
    skos:narrower F2021L00312:75 ;
    skos:prefLabel "Item I77"@en-AU ;
    dcat:accessURL <https://www.legislation.gov.au/F2021L00312/asmade/2021-03-24/text/original/epub/OEBPS/document_1/document_1.html#_Toc65843361> ;
    dcat:landingPage "https://www.legislation.gov.au/F2021L00312/asmade/2021-03-24/text/original/epub/OEBPS/document_1/document_1.html#_Toc65843361"^^xsd:anyURI ;
    dcat:theme legcons:Item .

F2021L00312:78 a legcons:Item,
        owl:Class,
        dcat:Resource ;
    rdfs:label "Item - I78 5 10  Measuring devices"@en-AU ;
    dct:isPartOf F2021L00312:75 ;
    dct:isReferencedBy F2021L00312: ;
    rdfs:comment "5 10  Measuring devices - Abrievated Graph Key: I78"@en-AU ;
    skos:definition "5 10  Measuring devices"@en-AU ;
    skos:narrower F2021L00312:75 ;
    skos:prefLabel "Item I78"@en-AU ;
    dcat:accessURL <https://www.legislation.gov.au/F2021L00312/asmade/2021-03-24/text/original/epub/OEBPS/document_1/document_1.html#_Toc65843362> ;
    dcat:landingPage "https://www.legislation.gov.au/F2021L00312/asmade/2021-03-24/text/original/epub/OEBPS/document_1/document_1.html#_Toc65843362"^^xsd:anyURI ;
    dcat:theme legcons:Item .

F2021L00312:79 a legcons:Item,
        owl:Class,
        dcat:Resource ;
    rdfs:label "Item - I79 5 11  Hygiene controlprocessing"@en-AU ;
    dct:isPartOf F2021L00312:75 ;
    dct:isReferencedBy F2021L00312: ;
    rdfs:comment "5 11  Hygiene controlprocessing - Abrievated Graph Key: I79"@en-AU ;
    skos:definition "5 11  Hygiene controlprocessing"@en-AU ;
    skos:narrower F2021L00312:75 ;
    skos:prefLabel "Item I79"@en-AU ;
    dcat:accessURL <https://www.legislation.gov.au/F2021L00312/asmade/2021-03-24/text/original/epub/OEBPS/document_1/document_1.html#_Toc65843363> ;
    dcat:landingPage "https://www.legislation.gov.au/F2021L00312/asmade/2021-03-24/text/original/epub/OEBPS/document_1/document_1.html#_Toc65843363"^^xsd:anyURI ;
    dcat:theme legcons:Item .

F2021L00312:8 a legcons:Item,
        owl:Class,
        dcat:Resource ;
    rdfs:label "Item - I8 1 5  Definitions"@en-AU ;
    dct:isPartOf F2021L00312:1 ;
    dct:isReferencedBy F2021L00312: ;
    rdfs:comment "1 5  Definitions - Abrievated Graph Key: I8"@en-AU ;
    skos:definition "1 5  Definitions"@en-AU ;
    skos:narrower F2021L00312:1 ;
    skos:prefLabel "Item I8"@en-AU ;
    dcat:accessURL <https://www.legislation.gov.au/F2021L00312/asmade/2021-03-24/text/original/epub/OEBPS/document_1/document_1.html#_Toc65843292> ;
    dcat:landingPage "https://www.legislation.gov.au/F2021L00312/asmade/2021-03-24/text/original/epub/OEBPS/document_1/document_1.html#_Toc65843292"^^xsd:anyURI ;
    dcat:theme legcons:Item .

F2021L00312:80 a legcons:Item,
        owl:Class,
        dcat:Resource ;
    rdfs:label "Item - I80 5 12  Personal hygiene and health"@en-AU ;
    dct:isPartOf F2021L00312:75 ;
    dct:isReferencedBy F2021L00312: ;
    rdfs:comment "5 12  Personal hygiene and health - Abrievated Graph Key: I80"@en-AU ;
    skos:definition "5 12  Personal hygiene and health"@en-AU ;
    skos:narrower F2021L00312:75 ;
    skos:prefLabel "Item I80"@en-AU ;
    dcat:accessURL <https://www.legislation.gov.au/F2021L00312/asmade/2021-03-24/text/original/epub/OEBPS/document_1/document_1.html#_Toc65843364> ;
    dcat:landingPage "https://www.legislation.gov.au/F2021L00312/asmade/2021-03-24/text/original/epub/OEBPS/document_1/document_1.html#_Toc65843364"^^xsd:anyURI ;
    dcat:theme legcons:Item .

F2021L00312:82 a legcons:Item,
        owl:Class,
        dcat:Resource ;
    rdfs:label "Item - I82 5 13  Sourcing eggs and egg products"@en-AU ;
    dct:isPartOf F2021L00312:81 ;
    dct:isReferencedBy F2021L00312: ;
    rdfs:comment "5 13  Sourcing eggs and egg products - Abrievated Graph Key: I82"@en-AU ;
    skos:definition "5 13  Sourcing eggs and egg products"@en-AU ;
    skos:narrower F2021L00312:81 ;
    skos:prefLabel "Item I82"@en-AU ;
    dcat:accessURL <https://www.legislation.gov.au/F2021L00312/asmade/2021-03-24/text/original/epub/OEBPS/document_1/document_1.html#_Toc65843366> ;
    dcat:landingPage "https://www.legislation.gov.au/F2021L00312/asmade/2021-03-24/text/original/epub/OEBPS/document_1/document_1.html#_Toc65843366"^^xsd:anyURI ;
    dcat:theme legcons:Item .

F2021L00312:83 a legcons:Item,
        owl:Class,
        dcat:Resource ;
    rdfs:label "Item - I83 5 14  Handling eggs and egg products"@en-AU ;
    dct:isPartOf F2021L00312:81 ;
    dct:isReferencedBy F2021L00312: ;
    rdfs:comment "5 14  Handling eggs and egg products - Abrievated Graph Key: I83"@en-AU ;
    skos:definition "5 14  Handling eggs and egg products"@en-AU ;
    skos:narrower F2021L00312:81 ;
    skos:prefLabel "Item I83"@en-AU ;
    dcat:accessURL <https://www.legislation.gov.au/F2021L00312/asmade/2021-03-24/text/original/epub/OEBPS/document_1/document_1.html#_Toc65843367> ;
    dcat:landingPage "https://www.legislation.gov.au/F2021L00312/asmade/2021-03-24/text/original/epub/OEBPS/document_1/document_1.html#_Toc65843367"^^xsd:anyURI ;
    dcat:theme legcons:Item .

F2021L00312:84 a legcons:Item,
        owl:Class,
        dcat:Resource ;
    rdfs:label "Item - I84 5 15  Notifiable diseases"@en-AU ;
    dct:isPartOf F2021L00312:81 ;
    dct:isReferencedBy F2021L00312: ;
    rdfs:comment "5 15  Notifiable diseases - Abrievated Graph Key: I84"@en-AU ;
    skos:definition "5 15  Notifiable diseases"@en-AU ;
    skos:narrower F2021L00312:81 ;
    skos:prefLabel "Item I84"@en-AU ;
    dcat:accessURL <https://www.legislation.gov.au/F2021L00312/asmade/2021-03-24/text/original/epub/OEBPS/document_1/document_1.html#_Toc65843368> ;
    dcat:landingPage "https://www.legislation.gov.au/F2021L00312/asmade/2021-03-24/text/original/epub/OEBPS/document_1/document_1.html#_Toc65843368"^^xsd:anyURI ;
    dcat:theme legcons:Item .

F2021L00312:85 a legcons:Item,
        owl:Class,
        dcat:Resource ;
    rdfs:label "Item - I85 5 16  Temperature controls for preparing prescribed eggs or egg products"@en-AU ;
    dct:isPartOf F2021L00312:81 ;
    dct:isReferencedBy F2021L00312: ;
    rdfs:comment "5 16  Temperature controls for preparing prescribed eggs or egg products - Abrievated Graph Key: I85"@en-AU ;
    skos:definition "5 16  Temperature controls for preparing prescribed eggs or egg products"@en-AU ;
    skos:narrower F2021L00312:81 ;
    skos:prefLabel "Item I85"@en-AU ;
    dcat:accessURL <https://www.legislation.gov.au/F2021L00312/asmade/2021-03-24/text/original/epub/OEBPS/document_1/document_1.html#_Toc65843369> ;
    dcat:landingPage "https://www.legislation.gov.au/F2021L00312/asmade/2021-03-24/text/original/epub/OEBPS/document_1/document_1.html#_Toc65843369"^^xsd:anyURI ;
    dcat:theme legcons:Item .

F2021L00312:86 a legcons:Item,
        owl:Class,
        dcat:Resource ;
    rdfs:label "Item - I86 5 17  Temperature controls for storing handling loading and transporting prescribed eggs or egg products"@en-AU ;
    dct:isPartOf F2021L00312:81 ;
    dct:isReferencedBy F2021L00312: ;
    rdfs:comment "5 17  Temperature controls for storing handling loading and transporting prescribed eggs or egg products - Abrievated Graph Key: I86"@en-AU ;
    skos:definition "5 17  Temperature controls for storing handling loading and transporting prescribed eggs or egg products"@en-AU ;
    skos:narrower F2021L00312:81 ;
    skos:prefLabel "Item I86"@en-AU ;
    dcat:accessURL <https://www.legislation.gov.au/F2021L00312/asmade/2021-03-24/text/original/epub/OEBPS/document_1/document_1.html#_Toc65843370> ;
    dcat:landingPage "https://www.legislation.gov.au/F2021L00312/asmade/2021-03-24/text/original/epub/OEBPS/document_1/document_1.html#_Toc65843370"^^xsd:anyURI ;
    dcat:theme legcons:Item .

F2021L00312:87 a legcons:Item,
        owl:Class,
        dcat:Resource ;
    rdfs:label "Item - I87 5 18  Preserving prescribed eggs and egg products"@en-AU ;
    dct:isPartOf F2021L00312:81 ;
    dct:isReferencedBy F2021L00312: ;
    rdfs:comment "5 18  Preserving prescribed eggs and egg products - Abrievated Graph Key: I87"@en-AU ;
    skos:definition "5 18  Preserving prescribed eggs and egg products"@en-AU ;
    skos:narrower F2021L00312:81 ;
    skos:prefLabel "Item I87"@en-AU ;
    dcat:accessURL <https://www.legislation.gov.au/F2021L00312/asmade/2021-03-24/text/original/epub/OEBPS/document_1/document_1.html#_Toc65843371> ;
    dcat:landingPage "https://www.legislation.gov.au/F2021L00312/asmade/2021-03-24/text/original/epub/OEBPS/document_1/document_1.html#_Toc65843371"^^xsd:anyURI ;
    dcat:theme legcons:Item .

F2021L00312:88 a legcons:Item,
        owl:Class,
        dcat:Resource ;
    rdfs:label "Item - I88 5 19  Thermal processing of canned prescribed eggs or egg products"@en-AU ;
    dct:isPartOf F2021L00312:81 ;
    dct:isReferencedBy F2021L00312: ;
    rdfs:comment "5 19  Thermal processing of canned prescribed eggs or egg products - Abrievated Graph Key: I88"@en-AU ;
    skos:definition "5 19  Thermal processing of canned prescribed eggs or egg products"@en-AU ;
    skos:narrower F2021L00312:81 ;
    skos:prefLabel "Item I88"@en-AU ;
    dcat:accessURL <https://www.legislation.gov.au/F2021L00312/asmade/2021-03-24/text/original/epub/OEBPS/document_1/document_1.html#_Toc65843372> ;
    dcat:landingPage "https://www.legislation.gov.au/F2021L00312/asmade/2021-03-24/text/original/epub/OEBPS/document_1/document_1.html#_Toc65843372"^^xsd:anyURI ;
    dcat:theme legcons:Item .

F2021L00312:89 a legcons:Item,
        owl:Class,
        dcat:Resource ;
    rdfs:label "Item - I89 5 20  Pasteurisation and other treatments"@en-AU ;
    dct:isPartOf F2021L00312:81 ;
    dct:isReferencedBy F2021L00312: ;
    rdfs:comment "5 20  Pasteurisation and other treatments - Abrievated Graph Key: I89"@en-AU ;
    skos:definition "5 20  Pasteurisation and other treatments"@en-AU ;
    skos:narrower F2021L00312:81 ;
    skos:prefLabel "Item I89"@en-AU ;
    dcat:accessURL <https://www.legislation.gov.au/F2021L00312/asmade/2021-03-24/text/original/epub/OEBPS/document_1/document_1.html#_Toc65843373> ;
    dcat:landingPage "https://www.legislation.gov.au/F2021L00312/asmade/2021-03-24/text/original/epub/OEBPS/document_1/document_1.html#_Toc65843373"^^xsd:anyURI ;
    dcat:theme legcons:Item .

F2021L00312:9 a legcons:Item,
        owl:Class,
        dcat:Resource ;
    rdfs:label "Item - I9 1 6  Meaning of loaded for export"@en-AU ;
    dct:isPartOf F2021L00312:1 ;
    dct:isReferencedBy F2021L00312: ;
    rdfs:comment "1 6  Meaning of loaded for export - Abrievated Graph Key: I9"@en-AU ;
    skos:definition "1 6  Meaning of loaded for export"@en-AU ;
    skos:narrower F2021L00312:1 ;
    skos:prefLabel "Item I9"@en-AU ;
    dcat:accessURL <https://www.legislation.gov.au/F2021L00312/asmade/2021-03-24/text/original/epub/OEBPS/document_1/document_1.html#_Toc65843293> ;
    dcat:landingPage "https://www.legislation.gov.au/F2021L00312/asmade/2021-03-24/text/original/epub/OEBPS/document_1/document_1.html#_Toc65843293"^^xsd:anyURI ;
    dcat:theme legcons:Item .

F2021L00312:90 a legcons:Item,
        owl:Class,
        dcat:Resource ;
    rdfs:label "Item - I90 5 21  Packaging and identification"@en-AU ;
    dct:isPartOf F2021L00312:81 ;
    dct:isReferencedBy F2021L00312: ;
    rdfs:comment "5 21  Packaging and identification - Abrievated Graph Key: I90"@en-AU ;
    skos:definition "5 21  Packaging and identification"@en-AU ;
    skos:narrower F2021L00312:81 ;
    skos:prefLabel "Item I90"@en-AU ;
    dcat:accessURL <https://www.legislation.gov.au/F2021L00312/asmade/2021-03-24/text/original/epub/OEBPS/document_1/document_1.html#_Toc65843374> ;
    dcat:landingPage "https://www.legislation.gov.au/F2021L00312/asmade/2021-03-24/text/original/epub/OEBPS/document_1/document_1.html#_Toc65843374"^^xsd:anyURI ;
    dcat:theme legcons:Item .

F2021L00312:91 a legcons:Item,
        owl:Class,
        dcat:Resource ;
    rdfs:label "Item - I91 5 22  Storage handling and loading"@en-AU ;
    dct:isPartOf F2021L00312:81 ;
    dct:isReferencedBy F2021L00312: ;
    rdfs:comment "5 22  Storage handling and loading - Abrievated Graph Key: I91"@en-AU ;
    skos:definition "5 22  Storage handling and loading"@en-AU ;
    skos:narrower F2021L00312:81 ;
    skos:prefLabel "Item I91"@en-AU ;
    dcat:accessURL <https://www.legislation.gov.au/F2021L00312/asmade/2021-03-24/text/original/epub/OEBPS/document_1/document_1.html#_Toc65843375> ;
    dcat:landingPage "https://www.legislation.gov.au/F2021L00312/asmade/2021-03-24/text/original/epub/OEBPS/document_1/document_1.html#_Toc65843375"^^xsd:anyURI ;
    dcat:theme legcons:Item .

F2021L00312:92 a legcons:Item,
        owl:Class,
        dcat:Resource ;
    rdfs:label "Item - I92 5 23  Container system units and food carrying compartments of vehiclesconstruction etc"@en-AU ;
    dct:isPartOf F2021L00312:81 ;
    dct:isReferencedBy F2021L00312: ;
    rdfs:comment "5 23  Container system units and food carrying compartments of vehiclesconstruction etc - Abrievated Graph Key: I92"@en-AU ;
    skos:definition "5 23  Container system units and food carrying compartments of vehiclesconstruction etc"@en-AU ;
    skos:narrower F2021L00312:81 ;
    skos:prefLabel "Item I92"@en-AU ;
    dcat:accessURL <https://www.legislation.gov.au/F2021L00312/asmade/2021-03-24/text/original/epub/OEBPS/document_1/document_1.html#_Toc65843376> ;
    dcat:landingPage "https://www.legislation.gov.au/F2021L00312/asmade/2021-03-24/text/original/epub/OEBPS/document_1/document_1.html#_Toc65843376"^^xsd:anyURI ;
    dcat:theme legcons:Item .

F2021L00312:93 a legcons:Item,
        owl:Class,
        dcat:Resource ;
    rdfs:label "Item - I93 5 24  Vehicles container system units etchygiene control"@en-AU ;
    dct:isPartOf F2021L00312:81 ;
    dct:isReferencedBy F2021L00312: ;
    rdfs:comment "5 24  Vehicles container system units etchygiene control - Abrievated Graph Key: I93"@en-AU ;
    skos:definition "5 24  Vehicles container system units etchygiene control"@en-AU ;
    skos:narrower F2021L00312:81 ;
    skos:prefLabel "Item I93"@en-AU ;
    dcat:accessURL <https://www.legislation.gov.au/F2021L00312/asmade/2021-03-24/text/original/epub/OEBPS/document_1/document_1.html#_Toc65843377> ;
    dcat:landingPage "https://www.legislation.gov.au/F2021L00312/asmade/2021-03-24/text/original/epub/OEBPS/document_1/document_1.html#_Toc65843377"^^xsd:anyURI ;
    dcat:theme legcons:Item .

F2021L00312:94 a legcons:Item,
        owl:Class,
        dcat:Resource ;
    rdfs:label "Item - I94 5 25  Transport"@en-AU ;
    dct:isPartOf F2021L00312:81 ;
    dct:isReferencedBy F2021L00312: ;
    rdfs:comment "5 25  Transport - Abrievated Graph Key: I94"@en-AU ;
    skos:definition "5 25  Transport"@en-AU ;
    skos:narrower F2021L00312:81 ;
    skos:prefLabel "Item I94"@en-AU ;
    dcat:accessURL <https://www.legislation.gov.au/F2021L00312/asmade/2021-03-24/text/original/epub/OEBPS/document_1/document_1.html#_Toc65843378> ;
    dcat:landingPage "https://www.legislation.gov.au/F2021L00312/asmade/2021-03-24/text/original/epub/OEBPS/document_1/document_1.html#_Toc65843378"^^xsd:anyURI ;
    dcat:theme legcons:Item .

F2021L00312:95 a legcons:Item,
        owl:Class,
        dcat:Resource ;
    rdfs:label "Item - I95 5 26  Identification as not for export as foodfitness for human consumption etc"@en-AU ;
    dct:isPartOf F2021L00312:81 ;
    dct:isReferencedBy F2021L00312: ;
    rdfs:comment "5 26  Identification as not for export as foodfitness for human consumption etc - Abrievated Graph Key: I95"@en-AU ;
    skos:definition "5 26  Identification as not for export as foodfitness for human consumption etc"@en-AU ;
    skos:narrower F2021L00312:81 ;
    skos:prefLabel "Item I95"@en-AU ;
    dcat:accessURL <https://www.legislation.gov.au/F2021L00312/asmade/2021-03-24/text/original/epub/OEBPS/document_1/document_1.html#_Toc65843379> ;
    dcat:landingPage "https://www.legislation.gov.au/F2021L00312/asmade/2021-03-24/text/original/epub/OEBPS/document_1/document_1.html#_Toc65843379"^^xsd:anyURI ;
    dcat:theme legcons:Item .

F2021L00312:96 a legcons:Item,
        owl:Class,
        dcat:Resource ;
    rdfs:label "Item - I96 5 27  Product standardsgeneral"@en-AU ;
    dct:isPartOf F2021L00312:81 ;
    dct:isReferencedBy F2021L00312: ;
    rdfs:comment "5 27  Product standardsgeneral - Abrievated Graph Key: I96"@en-AU ;
    skos:definition "5 27  Product standardsgeneral"@en-AU ;
    skos:narrower F2021L00312:81 ;
    skos:prefLabel "Item I96"@en-AU ;
    dcat:accessURL <https://www.legislation.gov.au/F2021L00312/asmade/2021-03-24/text/original/epub/OEBPS/document_1/document_1.html#_Toc65843380> ;
    dcat:landingPage "https://www.legislation.gov.au/F2021L00312/asmade/2021-03-24/text/original/epub/OEBPS/document_1/document_1.html#_Toc65843380"^^xsd:anyURI ;
    dcat:theme legcons:Item .

F2021L00312:98 a legcons:Item,
        owl:Class,
        dcat:Resource ;
    rdfs:label "Item - I98 5 28  Trade description must be applied to prescribed eggs and egg products"@en-AU ;
    dct:isPartOf F2021L00312:97 ;
    dct:isReferencedBy F2021L00312: ;
    rdfs:comment "5 28  Trade description must be applied to prescribed eggs and egg products - Abrievated Graph Key: I98"@en-AU ;
    skos:definition "5 28  Trade description must be applied to prescribed eggs and egg products"@en-AU ;
    skos:narrower F2021L00312:97 ;
    skos:prefLabel "Item I98"@en-AU ;
    dcat:accessURL <https://www.legislation.gov.au/F2021L00312/asmade/2021-03-24/text/original/epub/OEBPS/document_1/document_1.html#_Toc65843382> ;
    dcat:landingPage "https://www.legislation.gov.au/F2021L00312/asmade/2021-03-24/text/original/epub/OEBPS/document_1/document_1.html#_Toc65843382"^^xsd:anyURI ;
    dcat:theme legcons:Item .

F2021L00312:99 a legcons:Item,
        owl:Class,
        dcat:Resource ;
    rdfs:label "Item - I99 5 29  Incomplete trade descriptioncanned eggs or egg products"@en-AU ;
    dct:isPartOf F2021L00312:97 ;
    dct:isReferencedBy F2021L00312: ;
    rdfs:comment "5 29  Incomplete trade descriptioncanned eggs or egg products - Abrievated Graph Key: I99"@en-AU ;
    skos:definition "5 29  Incomplete trade descriptioncanned eggs or egg products"@en-AU ;
    skos:narrower F2021L00312:97 ;
    skos:prefLabel "Item I99"@en-AU ;
    dcat:accessURL <https://www.legislation.gov.au/F2021L00312/asmade/2021-03-24/text/original/epub/OEBPS/document_1/document_1.html#_Toc65843383> ;
    dcat:landingPage "https://www.legislation.gov.au/F2021L00312/asmade/2021-03-24/text/original/epub/OEBPS/document_1/document_1.html#_Toc65843383"^^xsd:anyURI ;
    dcat:theme legcons:Item .

F2021L00312:102 a legcons:Division,
        owl:Class,
        dcat:Resource ;
    rdfs:label "Division - D102 Division 6 Official marks"@en-AU ;
    dct:hasPart F2021L00312:103 ;
    dct:isPartOf F2021L00312:70 ;
    dct:isReferencedBy F2021L00312: ;
    rdfs:comment "Division 6 Official marks - Abrievated Graph Key: D102"@en-AU ;
    skos:broader F2021L00312:103 ;
    skos:definition "Division 6 Official marks"@en-AU ;
    skos:narrower F2021L00312:70 ;
    skos:prefLabel "Division D102"@en-AU ;
    dcat:accessURL <https://www.legislation.gov.au/F2021L00312/asmade/2021-03-24/text/original/epub/OEBPS/document_1/document_1.html#_Toc65843386> ;
    dcat:landingPage "https://www.legislation.gov.au/F2021L00312/asmade/2021-03-24/text/original/epub/OEBPS/document_1/document_1.html#_Toc65843386"^^xsd:anyURI ;
    dcat:theme legcons:Division .

F2021L00312:117 a legcons:Part,
        owl:Class,
        dcat:Resource ;
    rdfs:label "Part - P117 Part 3 Renewal of approved arrangement"@en-AU ;
    dct:hasPart F2021L00312:118 ;
    dct:isPartOf F2021L00312:63 ;
    dct:isReferencedBy F2021L00312: ;
    rdfs:comment "Part 3 Renewal of approved arrangement - Abrievated Graph Key: P117"@en-AU ;
    skos:broader F2021L00312:118 ;
    skos:definition "Part 3 Renewal of approved arrangement"@en-AU ;
    skos:narrower F2021L00312:63 ;
    skos:prefLabel "Part P117"@en-AU ;
    dcat:accessURL <https://www.legislation.gov.au/F2021L00312/asmade/2021-03-24/text/original/epub/OEBPS/document_1/document_1.html#_Toc65843401> ;
    dcat:landingPage "https://www.legislation.gov.au/F2021L00312/asmade/2021-03-24/text/original/epub/OEBPS/document_1/document_1.html#_Toc65843401"^^xsd:anyURI ;
    dcat:theme legcons:Part .

F2021L00312:123 a legcons:Division,
        owl:Class,
        dcat:Resource ;
    rdfs:label "Division - D123 Division 2 Variations required by Secretary"@en-AU ;
    dct:hasPart F2021L00312:124 ;
    dct:isPartOf F2021L00312:119 ;
    dct:isReferencedBy F2021L00312: ;
    rdfs:comment "Division 2 Variations required by Secretary - Abrievated Graph Key: D123"@en-AU ;
    skos:broader F2021L00312:124 ;
    skos:definition "Division 2 Variations required by Secretary"@en-AU ;
    skos:narrower F2021L00312:119 ;
    skos:prefLabel "Division D123"@en-AU ;
    dcat:accessURL <https://www.legislation.gov.au/F2021L00312/asmade/2021-03-24/text/original/epub/OEBPS/document_1/document_1.html#_Toc65843407> ;
    dcat:landingPage "https://www.legislation.gov.au/F2021L00312/asmade/2021-03-24/text/original/epub/OEBPS/document_1/document_1.html#_Toc65843407"^^xsd:anyURI ;
    dcat:theme legcons:Division .

F2021L00312:144 a legcons:Chapter,
        owl:Class,
        dcat:Resource ;
    rdfs:label "Chapter - C144 Chapter 8 Other matters relating to export"@en-AU ;
    dct:hasPart F2021L00312:145,
        F2021L00312:149 ;
    dct:isReferencedBy F2021L00312: ;
    rdfs:comment "Chapter 8 Other matters relating to export - Abrievated Graph Key: C144"@en-AU ;
    skos:broader F2021L00312:145,
        F2021L00312:149 ;
    skos:definition "Chapter 8 Other matters relating to export"@en-AU ;
    skos:prefLabel "Chapter C144"@en-AU ;
    dcat:accessURL <https://www.legislation.gov.au/F2021L00312/asmade/2021-03-24/text/original/epub/OEBPS/document_1/document_1.html#_Toc65843428> ;
    dcat:landingPage "https://www.legislation.gov.au/F2021L00312/asmade/2021-03-24/text/original/epub/OEBPS/document_1/document_1.html#_Toc65843428"^^xsd:anyURI ;
    dcat:theme legcons:Chapter .

F2021L00312:207 a legcons:Division,
        owl:Class,
        dcat:Resource ;
    rdfs:label "Division - D207 Division 1 General"@en-AU ;
    dct:hasPart F2021L00312:208 ;
    dct:isPartOf F2021L00312:206 ;
    dct:isReferencedBy F2021L00312: ;
    rdfs:comment "Division 1 General - Abrievated Graph Key: D207"@en-AU ;
    skos:broader F2021L00312:208 ;
    skos:definition "Division 1 General"@en-AU ;
    skos:narrower F2021L00312:206 ;
    skos:prefLabel "Division D207"@en-AU ;
    dcat:accessURL <https://www.legislation.gov.au/F2021L00312/asmade/2021-03-24/text/original/epub/OEBPS/document_1/document_1.html#_Toc65843491> ;
    dcat:landingPage "https://www.legislation.gov.au/F2021L00312/asmade/2021-03-24/text/original/epub/OEBPS/document_1/document_1.html#_Toc65843491"^^xsd:anyURI ;
    dcat:theme legcons:Division .

F2021L00312:224 a legcons:Part,
        owl:Class,
        dcat:Resource ;
    rdfs:label "Part - P224 Part 3 Powers of the Secretary"@en-AU ;
    dct:hasPart F2021L00312:225 ;
    dct:isPartOf F2021L00312:184 ;
    dct:isReferencedBy F2021L00312: ;
    rdfs:comment "Part 3 Powers of the Secretary - Abrievated Graph Key: P224"@en-AU ;
    skos:broader F2021L00312:225 ;
    skos:definition "Part 3 Powers of the Secretary"@en-AU ;
    skos:narrower F2021L00312:184 ;
    skos:prefLabel "Part P224"@en-AU ;
    dcat:accessURL <https://www.legislation.gov.au/F2021L00312/asmade/2021-03-24/text/original/epub/OEBPS/document_1/document_1.html#_Toc65843508> ;
    dcat:landingPage "https://www.legislation.gov.au/F2021L00312/asmade/2021-03-24/text/original/epub/OEBPS/document_1/document_1.html#_Toc65843508"^^xsd:anyURI ;
    dcat:theme legcons:Part .

F2021L00312:227 a legcons:Division,
        owl:Class,
        dcat:Resource ;
    rdfs:label "Division - D227 Division 1 Third party authorised officers"@en-AU ;
    dct:hasPart F2021L00312:228 ;
    dct:isPartOf F2021L00312:226 ;
    dct:isReferencedBy F2021L00312: ;
    rdfs:comment "Division 1 Third party authorised officers - Abrievated Graph Key: D227"@en-AU ;
    skos:broader F2021L00312:228 ;
    skos:definition "Division 1 Third party authorised officers"@en-AU ;
    skos:narrower F2021L00312:226 ;
    skos:prefLabel "Division D227"@en-AU ;
    dcat:accessURL <https://www.legislation.gov.au/F2021L00312/asmade/2021-03-24/text/original/epub/OEBPS/document_1/document_1.html#_Toc65843511> ;
    dcat:landingPage "https://www.legislation.gov.au/F2021L00312/asmade/2021-03-24/text/original/epub/OEBPS/document_1/document_1.html#_Toc65843511"^^xsd:anyURI ;
    dcat:theme legcons:Division .

F2021L00312:234 a legcons:Division,
        owl:Class,
        dcat:Resource ;
    rdfs:label "Division - D234 Division 3 Directions to deal with non compliance with the Act etc"@en-AU ;
    dct:hasPart F2021L00312:235 ;
    dct:isPartOf F2021L00312:226 ;
    dct:isReferencedBy F2021L00312: ;
    rdfs:comment "Division 3 Directions to deal with non compliance with the Act etc - Abrievated Graph Key: D234"@en-AU ;
    skos:broader F2021L00312:235 ;
    skos:definition "Division 3 Directions to deal with non compliance with the Act etc"@en-AU ;
    skos:narrower F2021L00312:226 ;
    skos:prefLabel "Division D234"@en-AU ;
    dcat:accessURL <https://www.legislation.gov.au/F2021L00312/asmade/2021-03-24/text/original/epub/OEBPS/document_1/document_1.html#_Toc65843518> ;
    dcat:landingPage "https://www.legislation.gov.au/F2021L00312/asmade/2021-03-24/text/original/epub/OEBPS/document_1/document_1.html#_Toc65843518"^^xsd:anyURI ;
    dcat:theme legcons:Division .

F2021L00312:236 a legcons:Division,
        owl:Class,
        dcat:Resource ;
    rdfs:label "Division - D236 Division 4 Miscellaneous"@en-AU ;
    dct:hasPart F2021L00312:237 ;
    dct:isPartOf F2021L00312:226 ;
    dct:isReferencedBy F2021L00312: ;
    rdfs:comment "Division 4 Miscellaneous - Abrievated Graph Key: D236"@en-AU ;
    skos:broader F2021L00312:237 ;
    skos:definition "Division 4 Miscellaneous"@en-AU ;
    skos:narrower F2021L00312:226 ;
    skos:prefLabel "Division D236"@en-AU ;
    dcat:accessURL <https://www.legislation.gov.au/F2021L00312/asmade/2021-03-24/text/original/epub/OEBPS/document_1/document_1.html#_Toc65843520> ;
    dcat:landingPage "https://www.legislation.gov.au/F2021L00312/asmade/2021-03-24/text/original/epub/OEBPS/document_1/document_1.html#_Toc65843520"^^xsd:anyURI ;
    dcat:theme legcons:Division .

F2021L00312:238 a legcons:Chapter,
        owl:Class,
        dcat:Resource ;
    rdfs:label "Chapter - C238 Chapter 10 Compliance and enforcement"@en-AU ;
    dct:hasPart F2021L00312:239,
        F2021L00312:240 ;
    dct:isReferencedBy F2021L00312: ;
    rdfs:comment "Chapter 10 Compliance and enforcement - Abrievated Graph Key: C238"@en-AU ;
    skos:broader F2021L00312:239,
        F2021L00312:240 ;
    skos:definition "Chapter 10 Compliance and enforcement"@en-AU ;
    skos:prefLabel "Chapter C238"@en-AU ;
    dcat:accessURL <https://www.legislation.gov.au/F2021L00312/asmade/2021-03-24/text/original/epub/OEBPS/document_1/document_1.html#_Toc65843522> ;
    dcat:landingPage "https://www.legislation.gov.au/F2021L00312/asmade/2021-03-24/text/original/epub/OEBPS/document_1/document_1.html#_Toc65843522"^^xsd:anyURI ;
    dcat:theme legcons:Chapter .

F2021L00312:242 a legcons:Part,
        owl:Class,
        dcat:Resource ;
    rdfs:label "Part - P242 Part 1 Review of decisions"@en-AU ;
    dct:hasPart F2021L00312:243 ;
    dct:isPartOf F2021L00312:241 ;
    dct:isReferencedBy F2021L00312: ;
    rdfs:comment "Part 1 Review of decisions - Abrievated Graph Key: P242"@en-AU ;
    skos:broader F2021L00312:243 ;
    skos:definition "Part 1 Review of decisions"@en-AU ;
    skos:narrower F2021L00312:241 ;
    skos:prefLabel "Part P242"@en-AU ;
    dcat:accessURL <https://www.legislation.gov.au/F2021L00312/asmade/2021-03-24/text/original/epub/OEBPS/document_1/document_1.html#_Toc65843526> ;
    dcat:landingPage "https://www.legislation.gov.au/F2021L00312/asmade/2021-03-24/text/original/epub/OEBPS/document_1/document_1.html#_Toc65843526"^^xsd:anyURI ;
    dcat:theme legcons:Part .

F2021L00312:260 a legcons:Part,
        owl:Class,
        dcat:Resource ;
    rdfs:label "Part - P260 Part 5 Relevant Commonwealth liabilities"@en-AU ;
    dct:hasPart F2021L00312:261 ;
    dct:isPartOf F2021L00312:241 ;
    dct:isReferencedBy F2021L00312: ;
    rdfs:comment "Part 5 Relevant Commonwealth liabilities - Abrievated Graph Key: P260"@en-AU ;
    skos:broader F2021L00312:261 ;
    skos:definition "Part 5 Relevant Commonwealth liabilities"@en-AU ;
    skos:narrower F2021L00312:241 ;
    skos:prefLabel "Part P260"@en-AU ;
    dcat:accessURL <https://www.legislation.gov.au/F2021L00312/asmade/2021-03-24/text/original/epub/OEBPS/document_1/document_1.html#_Toc65843544> ;
    dcat:landingPage "https://www.legislation.gov.au/F2021L00312/asmade/2021-03-24/text/original/epub/OEBPS/document_1/document_1.html#_Toc65843544"^^xsd:anyURI ;
    dcat:theme legcons:Part .

F2021L00312:263 a legcons:Part,
        owl:Class,
        dcat:Resource ;
    rdfs:label "Part - P263 Part 1 Preliminary"@en-AU ;
    dct:hasPart F2021L00312:264 ;
    dct:isPartOf F2021L00312:262 ;
    dct:isReferencedBy F2021L00312: ;
    rdfs:comment "Part 1 Preliminary - Abrievated Graph Key: P263"@en-AU ;
    skos:broader F2021L00312:264 ;
    skos:definition "Part 1 Preliminary"@en-AU ;
    skos:narrower F2021L00312:262 ;
    skos:prefLabel "Part P263"@en-AU ;
    dcat:accessURL <https://www.legislation.gov.au/F2021L00312/asmade/2021-03-24/text/original/epub/OEBPS/document_1/document_1.html#_Toc65843547> ;
    dcat:landingPage "https://www.legislation.gov.au/F2021L00312/asmade/2021-03-24/text/original/epub/OEBPS/document_1/document_1.html#_Toc65843547"^^xsd:anyURI ;
    dcat:theme legcons:Part .

F2021L00312:265 a legcons:Part,
        owl:Class,
        dcat:Resource ;
    rdfs:label "Part - P265 Part 2 Approved arrangements"@en-AU ;
    dct:hasPart F2021L00312:266 ;
    dct:isPartOf F2021L00312:262 ;
    dct:isReferencedBy F2021L00312: ;
    rdfs:comment "Part 2 Approved arrangements - Abrievated Graph Key: P265"@en-AU ;
    skos:broader F2021L00312:266 ;
    skos:definition "Part 2 Approved arrangements"@en-AU ;
    skos:narrower F2021L00312:262 ;
    skos:prefLabel "Part P265"@en-AU ;
    dcat:accessURL <https://www.legislation.gov.au/F2021L00312/asmade/2021-03-24/text/original/epub/OEBPS/document_1/document_1.html#_Toc65843549> ;
    dcat:landingPage "https://www.legislation.gov.au/F2021L00312/asmade/2021-03-24/text/original/epub/OEBPS/document_1/document_1.html#_Toc65843549"^^xsd:anyURI ;
    dcat:theme legcons:Part .

F2021L00312:268 a legcons:Division,
        owl:Class,
        dcat:Resource ;
    rdfs:label "Division - D268 Division 1 Trade descriptions"@en-AU ;
    dct:hasPart F2021L00312:269 ;
    dct:isPartOf F2021L00312:267 ;
    dct:isReferencedBy F2021L00312: ;
    rdfs:comment "Division 1 Trade descriptions - Abrievated Graph Key: D268"@en-AU ;
    skos:broader F2021L00312:269 ;
    skos:definition "Division 1 Trade descriptions"@en-AU ;
    skos:narrower F2021L00312:267 ;
    skos:prefLabel "Division D268"@en-AU ;
    dcat:accessURL <https://www.legislation.gov.au/F2021L00312/asmade/2021-03-24/text/original/epub/OEBPS/document_1/document_1.html#_Toc65843552> ;
    dcat:landingPage "https://www.legislation.gov.au/F2021L00312/asmade/2021-03-24/text/original/epub/OEBPS/document_1/document_1.html#_Toc65843552"^^xsd:anyURI ;
    dcat:theme legcons:Division .

F2021L00312:282 a legcons:Division,
        owl:Class,
        dcat:Resource ;
    rdfs:label "Division - D282 Division 2 Assessments"@en-AU ;
    dct:hasPart F2021L00312:283 ;
    dct:isPartOf F2021L00312:277 ;
    dct:isReferencedBy F2021L00312: ;
    rdfs:comment "Division 2 Assessments - Abrievated Graph Key: D282"@en-AU ;
    skos:broader F2021L00312:283 ;
    skos:definition "Division 2 Assessments"@en-AU ;
    skos:narrower F2021L00312:277 ;
    skos:prefLabel "Division D282"@en-AU ;
    dcat:accessURL <https://www.legislation.gov.au/F2021L00312/asmade/2021-03-24/text/original/epub/OEBPS/document_1/document_1.html#_Toc65843566> ;
    dcat:landingPage "https://www.legislation.gov.au/F2021L00312/asmade/2021-03-24/text/original/epub/OEBPS/document_1/document_1.html#_Toc65843566"^^xsd:anyURI ;
    dcat:theme legcons:Division .

F2021L00312:71 a legcons:Division,
        owl:Class,
        dcat:Resource ;
    rdfs:label "Division - D71 Division 1 Purpose of this Part"@en-AU ;
    dct:hasPart F2021L00312:72 ;
    dct:isPartOf F2021L00312:70 ;
    dct:isReferencedBy F2021L00312: ;
    rdfs:comment "Division 1 Purpose of this Part - Abrievated Graph Key: D71"@en-AU ;
    skos:broader F2021L00312:72 ;
    skos:definition "Division 1 Purpose of this Part"@en-AU ;
    skos:narrower F2021L00312:70 ;
    skos:prefLabel "Division D71"@en-AU ;
    dcat:accessURL <https://www.legislation.gov.au/F2021L00312/asmade/2021-03-24/text/original/epub/OEBPS/document_1/document_1.html#_Toc65843355> ;
    dcat:landingPage "https://www.legislation.gov.au/F2021L00312/asmade/2021-03-24/text/original/epub/OEBPS/document_1/document_1.html#_Toc65843355"^^xsd:anyURI ;
    dcat:theme legcons:Division .

F2021L00312:73 a legcons:Division,
        owl:Class,
        dcat:Resource ;
    rdfs:label "Division - D73 Division 2 General"@en-AU ;
    dct:hasPart F2021L00312:74 ;
    dct:isPartOf F2021L00312:70 ;
    dct:isReferencedBy F2021L00312: ;
    rdfs:comment "Division 2 General - Abrievated Graph Key: D73"@en-AU ;
    skos:broader F2021L00312:74 ;
    skos:definition "Division 2 General"@en-AU ;
    skos:narrower F2021L00312:70 ;
    skos:prefLabel "Division D73"@en-AU ;
    dcat:accessURL <https://www.legislation.gov.au/F2021L00312/asmade/2021-03-24/text/original/epub/OEBPS/document_1/document_1.html#_Toc65843357> ;
    dcat:landingPage "https://www.legislation.gov.au/F2021L00312/asmade/2021-03-24/text/original/epub/OEBPS/document_1/document_1.html#_Toc65843357"^^xsd:anyURI ;
    dcat:theme legcons:Division .

F2021L00312:108 a legcons:Division,
        owl:Class,
        dcat:Resource ;
    rdfs:label "Division - D108 Division 8 Transfers"@en-AU ;
    dct:hasPart F2021L00312:109,
        F2021L00312:110 ;
    dct:isPartOf F2021L00312:70 ;
    dct:isReferencedBy F2021L00312: ;
    rdfs:comment "Division 8 Transfers - Abrievated Graph Key: D108"@en-AU ;
    skos:broader F2021L00312:109,
        F2021L00312:110 ;
    skos:definition "Division 8 Transfers"@en-AU ;
    skos:narrower F2021L00312:70 ;
    skos:prefLabel "Division D108"@en-AU ;
    dcat:accessURL <https://www.legislation.gov.au/F2021L00312/asmade/2021-03-24/text/original/epub/OEBPS/document_1/document_1.html#_Toc65843392> ;
    dcat:landingPage "https://www.legislation.gov.au/F2021L00312/asmade/2021-03-24/text/original/epub/OEBPS/document_1/document_1.html#_Toc65843392"^^xsd:anyURI ;
    dcat:theme legcons:Division .

F2021L00312:119 a legcons:Part,
        owl:Class,
        dcat:Resource ;
    rdfs:label "Part - P119 Part 4 Variation of approved arrangement"@en-AU ;
    dct:hasPart F2021L00312:120,
        F2021L00312:123 ;
    dct:isPartOf F2021L00312:63 ;
    dct:isReferencedBy F2021L00312: ;
    rdfs:comment "Part 4 Variation of approved arrangement - Abrievated Graph Key: P119"@en-AU ;
    skos:broader F2021L00312:120,
        F2021L00312:123 ;
    skos:definition "Part 4 Variation of approved arrangement"@en-AU ;
    skos:narrower F2021L00312:63 ;
    skos:prefLabel "Part P119"@en-AU ;
    dcat:accessURL <https://www.legislation.gov.au/F2021L00312/asmade/2021-03-24/text/original/epub/OEBPS/document_1/document_1.html#_Toc65843403> ;
    dcat:landingPage "https://www.legislation.gov.au/F2021L00312/asmade/2021-03-24/text/original/epub/OEBPS/document_1/document_1.html#_Toc65843403"^^xsd:anyURI ;
    dcat:theme legcons:Part .

F2021L00312:12 a legcons:Division,
        owl:Class,
        dcat:Resource ;
    rdfs:label "Division - D12 Division 1 Prescribed goods"@en-AU ;
    dct:hasPart F2021L00312:13,
        F2021L00312:14 ;
    dct:isPartOf F2021L00312:11 ;
    dct:isReferencedBy F2021L00312: ;
    rdfs:comment "Division 1 Prescribed goods - Abrievated Graph Key: D12"@en-AU ;
    skos:broader F2021L00312:13,
        F2021L00312:14 ;
    skos:definition "Division 1 Prescribed goods"@en-AU ;
    skos:narrower F2021L00312:11 ;
    skos:prefLabel "Division D12"@en-AU ;
    dcat:accessURL <https://www.legislation.gov.au/F2021L00312/asmade/2021-03-24/text/original/epub/OEBPS/document_1/document_1.html#_Toc65843296> ;
    dcat:landingPage "https://www.legislation.gov.au/F2021L00312/asmade/2021-03-24/text/original/epub/OEBPS/document_1/document_1.html#_Toc65843296"^^xsd:anyURI ;
    dcat:theme legcons:Division .

F2021L00312:120 a legcons:Division,
        owl:Class,
        dcat:Resource ;
    rdfs:label "Division - D120 Division 1 Variations by holder"@en-AU ;
    dct:hasPart F2021L00312:121,
        F2021L00312:122 ;
    dct:isPartOf F2021L00312:119 ;
    dct:isReferencedBy F2021L00312: ;
    rdfs:comment "Division 1 Variations by holder - Abrievated Graph Key: D120"@en-AU ;
    skos:broader F2021L00312:121,
        F2021L00312:122 ;
    skos:definition "Division 1 Variations by holder"@en-AU ;
    skos:narrower F2021L00312:119 ;
    skos:prefLabel "Division D120"@en-AU ;
    dcat:accessURL <https://www.legislation.gov.au/F2021L00312/asmade/2021-03-24/text/original/epub/OEBPS/document_1/document_1.html#_Toc65843404> ;
    dcat:landingPage "https://www.legislation.gov.au/F2021L00312/asmade/2021-03-24/text/original/epub/OEBPS/document_1/document_1.html#_Toc65843404"^^xsd:anyURI ;
    dcat:theme legcons:Division .

F2021L00312:130 a legcons:Part,
        owl:Class,
        dcat:Resource ;
    rdfs:label "Part - P130 Part 1 Issue of export permit"@en-AU ;
    dct:hasPart F2021L00312:131,
        F2021L00312:132 ;
    dct:isPartOf F2021L00312:129 ;
    dct:isReferencedBy F2021L00312: ;
    rdfs:comment "Part 1 Issue of export permit - Abrievated Graph Key: P130"@en-AU ;
    skos:broader F2021L00312:131,
        F2021L00312:132 ;
    skos:definition "Part 1 Issue of export permit"@en-AU ;
    skos:narrower F2021L00312:129 ;
    skos:prefLabel "Part P130"@en-AU ;
    dcat:accessURL <https://www.legislation.gov.au/F2021L00312/asmade/2021-03-24/text/original/epub/OEBPS/document_1/document_1.html#_Toc65843414> ;
    dcat:landingPage "https://www.legislation.gov.au/F2021L00312/asmade/2021-03-24/text/original/epub/OEBPS/document_1/document_1.html#_Toc65843414"^^xsd:anyURI ;
    dcat:theme legcons:Part .

F2021L00312:141 a legcons:Part,
        owl:Class,
        dcat:Resource ;
    rdfs:label "Part - P141 Part 4 Applications for export permits"@en-AU ;
    dct:hasPart F2021L00312:142,
        F2021L00312:143 ;
    dct:isPartOf F2021L00312:129 ;
    dct:isReferencedBy F2021L00312: ;
    rdfs:comment "Part 4 Applications for export permits - Abrievated Graph Key: P141"@en-AU ;
    skos:broader F2021L00312:142,
        F2021L00312:143 ;
    skos:definition "Part 4 Applications for export permits"@en-AU ;
    skos:narrower F2021L00312:129 ;
    skos:prefLabel "Part P141"@en-AU ;
    dcat:accessURL <https://www.legislation.gov.au/F2021L00312/asmade/2021-03-24/text/original/epub/OEBPS/document_1/document_1.html#_Toc65843425> ;
    dcat:landingPage "https://www.legislation.gov.au/F2021L00312/asmade/2021-03-24/text/original/epub/OEBPS/document_1/document_1.html#_Toc65843425"^^xsd:anyURI ;
    dcat:theme legcons:Part .

F2021L00312:186 a legcons:Division,
        owl:Class,
        dcat:Resource ;
    rdfs:label "Division - D186 Division 1 General"@en-AU ;
    dct:hasPart F2021L00312:187,
        F2021L00312:188 ;
    dct:isPartOf F2021L00312:185 ;
    dct:isReferencedBy F2021L00312: ;
    rdfs:comment "Division 1 General - Abrievated Graph Key: D186"@en-AU ;
    skos:broader F2021L00312:187,
        F2021L00312:188 ;
    skos:definition "Division 1 General"@en-AU ;
    skos:narrower F2021L00312:185 ;
    skos:prefLabel "Division D186"@en-AU ;
    dcat:accessURL <https://www.legislation.gov.au/F2021L00312/asmade/2021-03-24/text/original/epub/OEBPS/document_1/document_1.html#_Toc65843470> ;
    dcat:landingPage "https://www.legislation.gov.au/F2021L00312/asmade/2021-03-24/text/original/epub/OEBPS/document_1/document_1.html#_Toc65843470"^^xsd:anyURI ;
    dcat:theme legcons:Division .

F2021L00312:209 a legcons:Division,
        owl:Class,
        dcat:Resource ;
    rdfs:label "Division - D209 Division 2 Carrying out assessments etc"@en-AU ;
    dct:hasPart F2021L00312:210,
        F2021L00312:211 ;
    dct:isPartOf F2021L00312:206 ;
    dct:isReferencedBy F2021L00312: ;
    rdfs:comment "Division 2 Carrying out assessments etc - Abrievated Graph Key: D209"@en-AU ;
    skos:broader F2021L00312:210,
        F2021L00312:211 ;
    skos:definition "Division 2 Carrying out assessments etc"@en-AU ;
    skos:narrower F2021L00312:206 ;
    skos:prefLabel "Division D209"@en-AU ;
    dcat:accessURL <https://www.legislation.gov.au/F2021L00312/asmade/2021-03-24/text/original/epub/OEBPS/document_1/document_1.html#_Toc65843493> ;
    dcat:landingPage "https://www.legislation.gov.au/F2021L00312/asmade/2021-03-24/text/original/epub/OEBPS/document_1/document_1.html#_Toc65843493"^^xsd:anyURI ;
    dcat:theme legcons:Division .

F2021L00312:254 a legcons:Part,
        owl:Class,
        dcat:Resource ;
    rdfs:label "Part - P254 Part 3 Samples"@en-AU ;
    dct:hasPart F2021L00312:255,
        F2021L00312:256 ;
    dct:isPartOf F2021L00312:241 ;
    dct:isReferencedBy F2021L00312: ;
    rdfs:comment "Part 3 Samples - Abrievated Graph Key: P254"@en-AU ;
    skos:broader F2021L00312:255,
        F2021L00312:256 ;
    skos:definition "Part 3 Samples"@en-AU ;
    skos:narrower F2021L00312:241 ;
    skos:prefLabel "Part P254"@en-AU ;
    dcat:accessURL <https://www.legislation.gov.au/F2021L00312/asmade/2021-03-24/text/original/epub/OEBPS/document_1/document_1.html#_Toc65843538> ;
    dcat:landingPage "https://www.legislation.gov.au/F2021L00312/asmade/2021-03-24/text/original/epub/OEBPS/document_1/document_1.html#_Toc65843538"^^xsd:anyURI ;
    dcat:theme legcons:Part .

F2021L00312:257 a legcons:Part,
        owl:Class,
        dcat:Resource ;
    rdfs:label "Part - P257 Part 4 Damaged or destroyed eggs or egg products"@en-AU ;
    dct:hasPart F2021L00312:258,
        F2021L00312:259 ;
    dct:isPartOf F2021L00312:241 ;
    dct:isReferencedBy F2021L00312: ;
    rdfs:comment "Part 4 Damaged or destroyed eggs or egg products - Abrievated Graph Key: P257"@en-AU ;
    skos:broader F2021L00312:258,
        F2021L00312:259 ;
    skos:definition "Part 4 Damaged or destroyed eggs or egg products"@en-AU ;
    skos:narrower F2021L00312:241 ;
    skos:prefLabel "Part P257"@en-AU ;
    dcat:accessURL <https://www.legislation.gov.au/F2021L00312/asmade/2021-03-24/text/original/epub/OEBPS/document_1/document_1.html#_Toc65843541> ;
    dcat:landingPage "https://www.legislation.gov.au/F2021L00312/asmade/2021-03-24/text/original/epub/OEBPS/document_1/document_1.html#_Toc65843541"^^xsd:anyURI ;
    dcat:theme legcons:Part .

F2021L00312:274 a legcons:Division,
        owl:Class,
        dcat:Resource ;
    rdfs:label "Division - D274 Division 3 Official marking devices"@en-AU ;
    dct:hasPart F2021L00312:275,
        F2021L00312:276 ;
    dct:isPartOf F2021L00312:267 ;
    dct:isReferencedBy F2021L00312: ;
    rdfs:comment "Division 3 Official marking devices - Abrievated Graph Key: D274"@en-AU ;
    skos:broader F2021L00312:275,
        F2021L00312:276 ;
    skos:definition "Division 3 Official marking devices"@en-AU ;
    skos:narrower F2021L00312:267 ;
    skos:prefLabel "Division D274"@en-AU ;
    dcat:accessURL <https://www.legislation.gov.au/F2021L00312/asmade/2021-03-24/text/original/epub/OEBPS/document_1/document_1.html#_Toc65843558> ;
    dcat:landingPage "https://www.legislation.gov.au/F2021L00312/asmade/2021-03-24/text/original/epub/OEBPS/document_1/document_1.html#_Toc65843558"^^xsd:anyURI ;
    dcat:theme legcons:Division .

F2021L00312:277 a legcons:Part,
        owl:Class,
        dcat:Resource ;
    rdfs:label "Part - P277 Part 4 Powers and officials"@en-AU ;
    dct:hasPart F2021L00312:278,
        F2021L00312:282 ;
    dct:isPartOf F2021L00312:262 ;
    dct:isReferencedBy F2021L00312: ;
    rdfs:comment "Part 4 Powers and officials - Abrievated Graph Key: P277"@en-AU ;
    skos:broader F2021L00312:278,
        F2021L00312:282 ;
    skos:definition "Part 4 Powers and officials"@en-AU ;
    skos:narrower F2021L00312:262 ;
    skos:prefLabel "Part P277"@en-AU ;
    dcat:accessURL <https://www.legislation.gov.au/F2021L00312/asmade/2021-03-24/text/original/epub/OEBPS/document_1/document_1.html#_Toc65843561> ;
    dcat:landingPage "https://www.legislation.gov.au/F2021L00312/asmade/2021-03-24/text/original/epub/OEBPS/document_1/document_1.html#_Toc65843561"^^xsd:anyURI ;
    dcat:theme legcons:Part .

F2021L00312:35 a legcons:Part,
        owl:Class,
        dcat:Resource ;
    rdfs:label "Part - P35 Part 1 Requirements for registration"@en-AU ;
    dct:hasPart F2021L00312:36,
        F2021L00312:46 ;
    dct:isPartOf F2021L00312:34 ;
    dct:isReferencedBy F2021L00312: ;
    rdfs:comment "Part 1 Requirements for registration - Abrievated Graph Key: P35"@en-AU ;
    skos:broader F2021L00312:36,
        F2021L00312:46 ;
    skos:definition "Part 1 Requirements for registration"@en-AU ;
    skos:narrower F2021L00312:34 ;
    skos:prefLabel "Part P35"@en-AU ;
    dcat:accessURL <https://www.legislation.gov.au/F2021L00312/asmade/2021-03-24/text/original/epub/OEBPS/document_1/document_1.html#_Toc65843319> ;
    dcat:landingPage "https://www.legislation.gov.au/F2021L00312/asmade/2021-03-24/text/original/epub/OEBPS/document_1/document_1.html#_Toc65843319"^^xsd:anyURI ;
    dcat:theme legcons:Part .

F2021L00312:46 a legcons:Division,
        owl:Class,
        dcat:Resource ;
    rdfs:label "Division - D46 Division 2 Other requirements"@en-AU ;
    dct:hasPart F2021L00312:47,
        F2021L00312:48 ;
    dct:isPartOf F2021L00312:35 ;
    dct:isReferencedBy F2021L00312: ;
    rdfs:comment "Division 2 Other requirements - Abrievated Graph Key: D46"@en-AU ;
    skos:broader F2021L00312:47,
        F2021L00312:48 ;
    skos:definition "Division 2 Other requirements"@en-AU ;
    skos:narrower F2021L00312:35 ;
    skos:prefLabel "Division D46"@en-AU ;
    dcat:accessURL <https://www.legislation.gov.au/F2021L00312/asmade/2021-03-24/text/original/epub/OEBPS/document_1/document_1.html#_Toc65843330> ;
    dcat:landingPage "https://www.legislation.gov.au/F2021L00312/asmade/2021-03-24/text/original/epub/OEBPS/document_1/document_1.html#_Toc65843330"^^xsd:anyURI ;
    dcat:theme legcons:Division .

F2021L00312:53 a legcons:Part,
        owl:Class,
        dcat:Resource ;
    rdfs:label "Part - P53 Part 3 Renewal of registration"@en-AU ;
    dct:hasPart F2021L00312:54,
        F2021L00312:55 ;
    dct:isPartOf F2021L00312:34 ;
    dct:isReferencedBy F2021L00312: ;
    rdfs:comment "Part 3 Renewal of registration - Abrievated Graph Key: P53"@en-AU ;
    skos:broader F2021L00312:54,
        F2021L00312:55 ;
    skos:definition "Part 3 Renewal of registration"@en-AU ;
    skos:narrower F2021L00312:34 ;
    skos:prefLabel "Part P53"@en-AU ;
    dcat:accessURL <https://www.legislation.gov.au/F2021L00312/asmade/2021-03-24/text/original/epub/OEBPS/document_1/document_1.html#_Toc65843337> ;
    dcat:landingPage "https://www.legislation.gov.au/F2021L00312/asmade/2021-03-24/text/original/epub/OEBPS/document_1/document_1.html#_Toc65843337"^^xsd:anyURI ;
    dcat:theme legcons:Part .

F2021L00312:56 a legcons:Part,
        owl:Class,
        dcat:Resource ;
    rdfs:label "Part - P56 Part 4 Suspension of registration"@en-AU ;
    dct:hasPart F2021L00312:57,
        F2021L00312:58 ;
    dct:isPartOf F2021L00312:34 ;
    dct:isReferencedBy F2021L00312: ;
    rdfs:comment "Part 4 Suspension of registration - Abrievated Graph Key: P56"@en-AU ;
    skos:broader F2021L00312:57,
        F2021L00312:58 ;
    skos:definition "Part 4 Suspension of registration"@en-AU ;
    skos:narrower F2021L00312:34 ;
    skos:prefLabel "Part P56"@en-AU ;
    dcat:accessURL <https://www.legislation.gov.au/F2021L00312/asmade/2021-03-24/text/original/epub/OEBPS/document_1/document_1.html#_Toc65843340> ;
    dcat:landingPage "https://www.legislation.gov.au/F2021L00312/asmade/2021-03-24/text/original/epub/OEBPS/document_1/document_1.html#_Toc65843340"^^xsd:anyURI ;
    dcat:theme legcons:Part .

F2021L00312:104 a legcons:Division,
        owl:Class,
        dcat:Resource ;
    rdfs:label "Division - D104 Division 7 Segregation identification security traceability and integrity"@en-AU ;
    dct:hasPart F2021L00312:105,
        F2021L00312:106,
        F2021L00312:107 ;
    dct:isPartOf F2021L00312:70 ;
    dct:isReferencedBy F2021L00312: ;
    rdfs:comment "Division 7 Segregation identification security traceability and integrity - Abrievated Graph Key: D104"@en-AU ;
    skos:broader F2021L00312:105,
        F2021L00312:106,
        F2021L00312:107 ;
    skos:definition "Division 7 Segregation identification security traceability and integrity"@en-AU ;
    skos:narrower F2021L00312:70 ;
    skos:prefLabel "Division D104"@en-AU ;
    dcat:accessURL <https://www.legislation.gov.au/F2021L00312/asmade/2021-03-24/text/original/epub/OEBPS/document_1/document_1.html#_Toc65843388> ;
    dcat:landingPage "https://www.legislation.gov.au/F2021L00312/asmade/2021-03-24/text/original/epub/OEBPS/document_1/document_1.html#_Toc65843388"^^xsd:anyURI ;
    dcat:theme legcons:Division .

F2021L00312:125 a legcons:Part,
        owl:Class,
        dcat:Resource ;
    rdfs:label "Part - P125 Part 5 Matters relating to applications"@en-AU ;
    dct:hasPart F2021L00312:126,
        F2021L00312:127,
        F2021L00312:128 ;
    dct:isPartOf F2021L00312:63 ;
    dct:isReferencedBy F2021L00312: ;
    rdfs:comment "Part 5 Matters relating to applications - Abrievated Graph Key: P125"@en-AU ;
    skos:broader F2021L00312:126,
        F2021L00312:127,
        F2021L00312:128 ;
    skos:definition "Part 5 Matters relating to applications"@en-AU ;
    skos:narrower F2021L00312:63 ;
    skos:prefLabel "Part P125"@en-AU ;
    dcat:accessURL <https://www.legislation.gov.au/F2021L00312/asmade/2021-03-24/text/original/epub/OEBPS/document_1/document_1.html#_Toc65843409> ;
    dcat:landingPage "https://www.legislation.gov.au/F2021L00312/asmade/2021-03-24/text/original/epub/OEBPS/document_1/document_1.html#_Toc65843409"^^xsd:anyURI ;
    dcat:theme legcons:Part .

F2021L00312:129 a legcons:Chapter,
        owl:Class,
        dcat:Resource ;
    rdfs:label "Chapter - C129 Chapter 7 Export permits"@en-AU ;
    dct:hasPart F2021L00312:130,
        F2021L00312:133,
        F2021L00312:137,
        F2021L00312:141 ;
    dct:isReferencedBy F2021L00312: ;
    rdfs:comment "Chapter 7 Export permits - Abrievated Graph Key: C129"@en-AU ;
    skos:broader F2021L00312:130,
        F2021L00312:133,
        F2021L00312:137,
        F2021L00312:141 ;
    skos:definition "Chapter 7 Export permits"@en-AU ;
    skos:prefLabel "Chapter C129"@en-AU ;
    dcat:accessURL <https://www.legislation.gov.au/F2021L00312/asmade/2021-03-24/text/original/epub/OEBPS/document_1/document_1.html#_Toc65843413> ;
    dcat:landingPage "https://www.legislation.gov.au/F2021L00312/asmade/2021-03-24/text/original/epub/OEBPS/document_1/document_1.html#_Toc65843413"^^xsd:anyURI ;
    dcat:theme legcons:Chapter .

F2021L00312:133 a legcons:Part,
        owl:Class,
        dcat:Resource ;
    rdfs:label "Part - P133 Part 2 Variation suspension and revocation of export permit"@en-AU ;
    dct:hasPart F2021L00312:134,
        F2021L00312:135,
        F2021L00312:136 ;
    dct:isPartOf F2021L00312:129 ;
    dct:isReferencedBy F2021L00312: ;
    rdfs:comment "Part 2 Variation suspension and revocation of export permit - Abrievated Graph Key: P133"@en-AU ;
    skos:broader F2021L00312:134,
        F2021L00312:135,
        F2021L00312:136 ;
    skos:definition "Part 2 Variation suspension and revocation of export permit"@en-AU ;
    skos:narrower F2021L00312:129 ;
    skos:prefLabel "Part P133"@en-AU ;
    dcat:accessURL <https://www.legislation.gov.au/F2021L00312/asmade/2021-03-24/text/original/epub/OEBPS/document_1/document_1.html#_Toc65843417> ;
    dcat:landingPage "https://www.legislation.gov.au/F2021L00312/asmade/2021-03-24/text/original/epub/OEBPS/document_1/document_1.html#_Toc65843417"^^xsd:anyURI ;
    dcat:theme legcons:Part .

F2021L00312:137 a legcons:Part,
        owl:Class,
        dcat:Resource ;
    rdfs:label "Part - P137 Part 3 Other matters"@en-AU ;
    dct:hasPart F2021L00312:138,
        F2021L00312:139,
        F2021L00312:140 ;
    dct:isPartOf F2021L00312:129 ;
    dct:isReferencedBy F2021L00312: ;
    rdfs:comment "Part 3 Other matters - Abrievated Graph Key: P137"@en-AU ;
    skos:broader F2021L00312:138,
        F2021L00312:139,
        F2021L00312:140 ;
    skos:definition "Part 3 Other matters"@en-AU ;
    skos:narrower F2021L00312:129 ;
    skos:prefLabel "Part P137"@en-AU ;
    dcat:accessURL <https://www.legislation.gov.au/F2021L00312/asmade/2021-03-24/text/original/epub/OEBPS/document_1/document_1.html#_Toc65843421> ;
    dcat:landingPage "https://www.legislation.gov.au/F2021L00312/asmade/2021-03-24/text/original/epub/OEBPS/document_1/document_1.html#_Toc65843421"^^xsd:anyURI ;
    dcat:theme legcons:Part .

F2021L00312:145 a legcons:Part,
        owl:Class,
        dcat:Resource ;
    rdfs:label "Part - P145 Part 1 Trade descriptions"@en-AU ;
    dct:hasPart F2021L00312:146,
        F2021L00312:147,
        F2021L00312:148 ;
    dct:isPartOf F2021L00312:144 ;
    dct:isReferencedBy F2021L00312: ;
    rdfs:comment "Part 1 Trade descriptions - Abrievated Graph Key: P145"@en-AU ;
    skos:broader F2021L00312:146,
        F2021L00312:147,
        F2021L00312:148 ;
    skos:definition "Part 1 Trade descriptions"@en-AU ;
    skos:narrower F2021L00312:144 ;
    skos:prefLabel "Part P145"@en-AU ;
    dcat:accessURL <https://www.legislation.gov.au/F2021L00312/asmade/2021-03-24/text/original/epub/OEBPS/document_1/document_1.html#_Toc65843429> ;
    dcat:landingPage "https://www.legislation.gov.au/F2021L00312/asmade/2021-03-24/text/original/epub/OEBPS/document_1/document_1.html#_Toc65843429"^^xsd:anyURI ;
    dcat:theme legcons:Part .

F2021L00312:173 a legcons:Division,
        owl:Class,
        dcat:Resource ;
    rdfs:label "Division - D173 Division 3 Marks resembling official marks"@en-AU ;
    dct:hasPart F2021L00312:174,
        F2021L00312:175,
        F2021L00312:176 ;
    dct:isPartOf F2021L00312:149 ;
    dct:isReferencedBy F2021L00312: ;
    rdfs:comment "Division 3 Marks resembling official marks - Abrievated Graph Key: D173"@en-AU ;
    skos:broader F2021L00312:174,
        F2021L00312:175,
        F2021L00312:176 ;
    skos:definition "Division 3 Marks resembling official marks"@en-AU ;
    skos:narrower F2021L00312:149 ;
    skos:prefLabel "Division D173"@en-AU ;
    dcat:accessURL <https://www.legislation.gov.au/F2021L00312/asmade/2021-03-24/text/original/epub/OEBPS/document_1/document_1.html#_Toc65843457> ;
    dcat:landingPage "https://www.legislation.gov.au/F2021L00312/asmade/2021-03-24/text/original/epub/OEBPS/document_1/document_1.html#_Toc65843457"^^xsd:anyURI ;
    dcat:theme legcons:Division .

F2021L00312:184 a legcons:Chapter,
        owl:Class,
        dcat:Resource ;
    rdfs:label "Chapter - C184 Chapter 9 Powers and officials"@en-AU ;
    dct:hasPart F2021L00312:185,
        F2021L00312:206,
        F2021L00312:224,
        F2021L00312:226 ;
    dct:isReferencedBy F2021L00312: ;
    rdfs:comment "Chapter 9 Powers and officials - Abrievated Graph Key: C184"@en-AU ;
    skos:broader F2021L00312:185,
        F2021L00312:206,
        F2021L00312:224,
        F2021L00312:226 ;
    skos:definition "Chapter 9 Powers and officials"@en-AU ;
    skos:prefLabel "Chapter C184"@en-AU ;
    dcat:accessURL <https://www.legislation.gov.au/F2021L00312/asmade/2021-03-24/text/original/epub/OEBPS/document_1/document_1.html#_Toc65843468> ;
    dcat:landingPage "https://www.legislation.gov.au/F2021L00312/asmade/2021-03-24/text/original/epub/OEBPS/document_1/document_1.html#_Toc65843468"^^xsd:anyURI ;
    dcat:theme legcons:Chapter .

F2021L00312:185 a legcons:Part,
        owl:Class,
        dcat:Resource ;
    rdfs:label "Part - P185 Part 1 Audits"@en-AU ;
    dct:hasPart F2021L00312:186,
        F2021L00312:189,
        F2021L00312:194 ;
    dct:isPartOf F2021L00312:184 ;
    dct:isReferencedBy F2021L00312: ;
    rdfs:comment "Part 1 Audits - Abrievated Graph Key: P185"@en-AU ;
    skos:broader F2021L00312:186,
        F2021L00312:189,
        F2021L00312:194 ;
    skos:definition "Part 1 Audits"@en-AU ;
    skos:narrower F2021L00312:184 ;
    skos:prefLabel "Part P185"@en-AU ;
    dcat:accessURL <https://www.legislation.gov.au/F2021L00312/asmade/2021-03-24/text/original/epub/OEBPS/document_1/document_1.html#_Toc65843469> ;
    dcat:landingPage "https://www.legislation.gov.au/F2021L00312/asmade/2021-03-24/text/original/epub/OEBPS/document_1/document_1.html#_Toc65843469"^^xsd:anyURI ;
    dcat:theme legcons:Part .

F2021L00312:206 a legcons:Part,
        owl:Class,
        dcat:Resource ;
    rdfs:label "Part - P206 Part 2 Assessments"@en-AU ;
    dct:hasPart F2021L00312:207,
        F2021L00312:209,
        F2021L00312:212 ;
    dct:isPartOf F2021L00312:184 ;
    dct:isReferencedBy F2021L00312: ;
    rdfs:comment "Part 2 Assessments - Abrievated Graph Key: P206"@en-AU ;
    skos:broader F2021L00312:207,
        F2021L00312:209,
        F2021L00312:212 ;
    skos:definition "Part 2 Assessments"@en-AU ;
    skos:narrower F2021L00312:184 ;
    skos:prefLabel "Part P206"@en-AU ;
    dcat:accessURL <https://www.legislation.gov.au/F2021L00312/asmade/2021-03-24/text/original/epub/OEBPS/document_1/document_1.html#_Toc65843490> ;
    dcat:landingPage "https://www.legislation.gov.au/F2021L00312/asmade/2021-03-24/text/original/epub/OEBPS/document_1/document_1.html#_Toc65843490"^^xsd:anyURI ;
    dcat:theme legcons:Part .

F2021L00312:262 a legcons:Chapter,
        owl:Class,
        dcat:Resource ;
    rdfs:label "Chapter - C262 Chapter 12 Transitional provisions"@en-AU ;
    dct:hasPart F2021L00312:263,
        F2021L00312:265,
        F2021L00312:267,
        F2021L00312:277 ;
    dct:isReferencedBy F2021L00312: ;
    rdfs:comment "Chapter 12 Transitional provisions - Abrievated Graph Key: C262"@en-AU ;
    skos:broader F2021L00312:263,
        F2021L00312:265,
        F2021L00312:267,
        F2021L00312:277 ;
    skos:definition "Chapter 12 Transitional provisions"@en-AU ;
    skos:prefLabel "Chapter C262"@en-AU ;
    dcat:accessURL <https://www.legislation.gov.au/F2021L00312/asmade/2021-03-24/text/original/epub/OEBPS/document_1/document_1.html#_Toc65843546> ;
    dcat:landingPage "https://www.legislation.gov.au/F2021L00312/asmade/2021-03-24/text/original/epub/OEBPS/document_1/document_1.html#_Toc65843546"^^xsd:anyURI ;
    dcat:theme legcons:Chapter .

F2021L00312:267 a legcons:Part,
        owl:Class,
        dcat:Resource ;
    rdfs:label "Part - P267 Part 3 Other matters relating to export"@en-AU ;
    dct:hasPart F2021L00312:268,
        F2021L00312:270,
        F2021L00312:274 ;
    dct:isPartOf F2021L00312:262 ;
    dct:isReferencedBy F2021L00312: ;
    rdfs:comment "Part 3 Other matters relating to export - Abrievated Graph Key: P267"@en-AU ;
    skos:broader F2021L00312:268,
        F2021L00312:270,
        F2021L00312:274 ;
    skos:definition "Part 3 Other matters relating to export"@en-AU ;
    skos:narrower F2021L00312:262 ;
    skos:prefLabel "Part P267"@en-AU ;
    dcat:accessURL <https://www.legislation.gov.au/F2021L00312/asmade/2021-03-24/text/original/epub/OEBPS/document_1/document_1.html#_Toc65843551> ;
    dcat:landingPage "https://www.legislation.gov.au/F2021L00312/asmade/2021-03-24/text/original/epub/OEBPS/document_1/document_1.html#_Toc65843551"^^xsd:anyURI ;
    dcat:theme legcons:Part .

F2021L00312:270 a legcons:Division,
        owl:Class,
        dcat:Resource ;
    rdfs:label "Division - D270 Division 2 Official marks"@en-AU ;
    dct:hasPart F2021L00312:271,
        F2021L00312:272,
        F2021L00312:273 ;
    dct:isPartOf F2021L00312:267 ;
    dct:isReferencedBy F2021L00312: ;
    rdfs:comment "Division 2 Official marks - Abrievated Graph Key: D270"@en-AU ;
    skos:broader F2021L00312:271,
        F2021L00312:272,
        F2021L00312:273 ;
    skos:definition "Division 2 Official marks"@en-AU ;
    skos:narrower F2021L00312:267 ;
    skos:prefLabel "Division D270"@en-AU ;
    dcat:accessURL <https://www.legislation.gov.au/F2021L00312/asmade/2021-03-24/text/original/epub/OEBPS/document_1/document_1.html#_Toc65843554> ;
    dcat:landingPage "https://www.legislation.gov.au/F2021L00312/asmade/2021-03-24/text/original/epub/OEBPS/document_1/document_1.html#_Toc65843554"^^xsd:anyURI ;
    dcat:theme legcons:Division .

F2021L00312:278 a legcons:Division,
        owl:Class,
        dcat:Resource ;
    rdfs:label "Division - D278 Division 1 Approved auditors"@en-AU ;
    dct:hasPart F2021L00312:279,
        F2021L00312:280,
        F2021L00312:281 ;
    dct:isPartOf F2021L00312:277 ;
    dct:isReferencedBy F2021L00312: ;
    rdfs:comment "Division 1 Approved auditors - Abrievated Graph Key: D278"@en-AU ;
    skos:broader F2021L00312:279,
        F2021L00312:280,
        F2021L00312:281 ;
    skos:definition "Division 1 Approved auditors"@en-AU ;
    skos:narrower F2021L00312:277 ;
    skos:prefLabel "Division D278"@en-AU ;
    dcat:accessURL <https://www.legislation.gov.au/F2021L00312/asmade/2021-03-24/text/original/epub/OEBPS/document_1/document_1.html#_Toc65843562> ;
    dcat:landingPage "https://www.legislation.gov.au/F2021L00312/asmade/2021-03-24/text/original/epub/OEBPS/document_1/document_1.html#_Toc65843562"^^xsd:anyURI ;
    dcat:theme legcons:Division .

F2021L00312:49 a legcons:Part,
        owl:Class,
        dcat:Resource ;
    rdfs:label "Part - P49 Part 2 Conditions of registration"@en-AU ;
    dct:hasPart F2021L00312:50,
        F2021L00312:51,
        F2021L00312:52 ;
    dct:isPartOf F2021L00312:34 ;
    dct:isReferencedBy F2021L00312: ;
    rdfs:comment "Part 2 Conditions of registration - Abrievated Graph Key: P49"@en-AU ;
    skos:broader F2021L00312:50,
        F2021L00312:51,
        F2021L00312:52 ;
    skos:definition "Part 2 Conditions of registration"@en-AU ;
    skos:narrower F2021L00312:34 ;
    skos:prefLabel "Part P49"@en-AU ;
    dcat:accessURL <https://www.legislation.gov.au/F2021L00312/asmade/2021-03-24/text/original/epub/OEBPS/document_1/document_1.html#_Toc65843333> ;
    dcat:landingPage "https://www.legislation.gov.au/F2021L00312/asmade/2021-03-24/text/original/epub/OEBPS/document_1/document_1.html#_Toc65843333"^^xsd:anyURI ;
    dcat:theme legcons:Part .

F2021L00312:59 a legcons:Part,
        owl:Class,
        dcat:Resource ;
    rdfs:label "Part - P59 Part 5 Matters relating to applications"@en-AU ;
    dct:hasPart F2021L00312:60,
        F2021L00312:61,
        F2021L00312:62 ;
    dct:isPartOf F2021L00312:34 ;
    dct:isReferencedBy F2021L00312: ;
    rdfs:comment "Part 5 Matters relating to applications - Abrievated Graph Key: P59"@en-AU ;
    skos:broader F2021L00312:60,
        F2021L00312:61,
        F2021L00312:62 ;
    skos:definition "Part 5 Matters relating to applications"@en-AU ;
    skos:narrower F2021L00312:34 ;
    skos:prefLabel "Part P59"@en-AU ;
    dcat:accessURL <https://www.legislation.gov.au/F2021L00312/asmade/2021-03-24/text/original/epub/OEBPS/document_1/document_1.html#_Toc65843343> ;
    dcat:landingPage "https://www.legislation.gov.au/F2021L00312/asmade/2021-03-24/text/original/epub/OEBPS/document_1/document_1.html#_Toc65843343"^^xsd:anyURI ;
    dcat:theme legcons:Part .

F2021L00312:11 a legcons:Part,
        owl:Class,
        dcat:Resource ;
    rdfs:label "Part - P11 Part 1 Goods"@en-AU ;
    dct:hasPart F2021L00312:12,
        F2021L00312:15,
        F2021L00312:16,
        F2021L00312:17 ;
    dct:isPartOf F2021L00312:10 ;
    dct:isReferencedBy F2021L00312: ;
    rdfs:comment "Part 1 Goods - Abrievated Graph Key: P11"@en-AU ;
    skos:broader F2021L00312:12,
        F2021L00312:15,
        F2021L00312:16,
        F2021L00312:17 ;
    skos:definition "Part 1 Goods"@en-AU ;
    skos:narrower F2021L00312:10 ;
    skos:prefLabel "Part P11"@en-AU ;
    dcat:accessURL <https://www.legislation.gov.au/F2021L00312/asmade/2021-03-24/text/original/epub/OEBPS/document_1/document_1.html#_Toc65843295> ;
    dcat:landingPage "https://www.legislation.gov.au/F2021L00312/asmade/2021-03-24/text/original/epub/OEBPS/document_1/document_1.html#_Toc65843295"^^xsd:anyURI ;
    dcat:theme legcons:Part .

F2021L00312:149 a legcons:Part,
        owl:Class,
        dcat:Resource ;
    rdfs:label "Part - P149 Part 2 Official marks"@en-AU ;
    dct:hasPart F2021L00312:150,
        F2021L00312:160,
        F2021L00312:173,
        F2021L00312:177 ;
    dct:isPartOf F2021L00312:144 ;
    dct:isReferencedBy F2021L00312: ;
    rdfs:comment "Part 2 Official marks - Abrievated Graph Key: P149"@en-AU ;
    skos:broader F2021L00312:150,
        F2021L00312:160,
        F2021L00312:173,
        F2021L00312:177 ;
    skos:definition "Part 2 Official marks"@en-AU ;
    skos:narrower F2021L00312:144 ;
    skos:prefLabel "Part P149"@en-AU ;
    dcat:accessURL <https://www.legislation.gov.au/F2021L00312/asmade/2021-03-24/text/original/epub/OEBPS/document_1/document_1.html#_Toc65843433> ;
    dcat:landingPage "https://www.legislation.gov.au/F2021L00312/asmade/2021-03-24/text/original/epub/OEBPS/document_1/document_1.html#_Toc65843433"^^xsd:anyURI ;
    dcat:theme legcons:Part .

F2021L00312:189 a legcons:Division,
        owl:Class,
        dcat:Resource ;
    rdfs:label "Division - D189 Division 2 Conduct of audit etc"@en-AU ;
    dct:hasPart F2021L00312:190,
        F2021L00312:191,
        F2021L00312:192,
        F2021L00312:193 ;
    dct:isPartOf F2021L00312:185 ;
    dct:isReferencedBy F2021L00312: ;
    rdfs:comment "Division 2 Conduct of audit etc - Abrievated Graph Key: D189"@en-AU ;
    skos:broader F2021L00312:190,
        F2021L00312:191,
        F2021L00312:192,
        F2021L00312:193 ;
    skos:definition "Division 2 Conduct of audit etc"@en-AU ;
    skos:narrower F2021L00312:185 ;
    skos:prefLabel "Division D189"@en-AU ;
    dcat:accessURL <https://www.legislation.gov.au/F2021L00312/asmade/2021-03-24/text/original/epub/OEBPS/document_1/document_1.html#_Toc65843473> ;
    dcat:landingPage "https://www.legislation.gov.au/F2021L00312/asmade/2021-03-24/text/original/epub/OEBPS/document_1/document_1.html#_Toc65843473"^^xsd:anyURI ;
    dcat:theme legcons:Division .

F2021L00312:226 a legcons:Part,
        owl:Class,
        dcat:Resource ;
    rdfs:label "Part - P226 Part 4 Authorised officers"@en-AU ;
    dct:hasPart F2021L00312:227,
        F2021L00312:229,
        F2021L00312:234,
        F2021L00312:236 ;
    dct:isPartOf F2021L00312:184 ;
    dct:isReferencedBy F2021L00312: ;
    rdfs:comment "Part 4 Authorised officers - Abrievated Graph Key: P226"@en-AU ;
    skos:broader F2021L00312:227,
        F2021L00312:229,
        F2021L00312:234,
        F2021L00312:236 ;
    skos:definition "Part 4 Authorised officers"@en-AU ;
    skos:narrower F2021L00312:184 ;
    skos:prefLabel "Part P226"@en-AU ;
    dcat:accessURL <https://www.legislation.gov.au/F2021L00312/asmade/2021-03-24/text/original/epub/OEBPS/document_1/document_1.html#_Toc65843510> ;
    dcat:landingPage "https://www.legislation.gov.au/F2021L00312/asmade/2021-03-24/text/original/epub/OEBPS/document_1/document_1.html#_Toc65843510"^^xsd:anyURI ;
    dcat:theme legcons:Part .

F2021L00312:229 a legcons:Division,
        owl:Class,
        dcat:Resource ;
    rdfs:label "Division - D229 Division 2 Functions and powers"@en-AU ;
    dct:hasPart F2021L00312:230,
        F2021L00312:231,
        F2021L00312:232,
        F2021L00312:233 ;
    dct:isPartOf F2021L00312:226 ;
    dct:isReferencedBy F2021L00312: ;
    rdfs:comment "Division 2 Functions and powers - Abrievated Graph Key: D229"@en-AU ;
    skos:broader F2021L00312:230,
        F2021L00312:231,
        F2021L00312:232,
        F2021L00312:233 ;
    skos:definition "Division 2 Functions and powers"@en-AU ;
    skos:narrower F2021L00312:226 ;
    skos:prefLabel "Division D229"@en-AU ;
    dcat:accessURL <https://www.legislation.gov.au/F2021L00312/asmade/2021-03-24/text/original/epub/OEBPS/document_1/document_1.html#_Toc65843513> ;
    dcat:landingPage "https://www.legislation.gov.au/F2021L00312/asmade/2021-03-24/text/original/epub/OEBPS/document_1/document_1.html#_Toc65843513"^^xsd:anyURI ;
    dcat:theme legcons:Division .

F2021L00312:241 a legcons:Chapter,
        owl:Class,
        dcat:Resource ;
    rdfs:label "Chapter - C241 Chapter 11 Miscellaneous"@en-AU ;
    dct:hasPart F2021L00312:242,
        F2021L00312:244,
        F2021L00312:254,
        F2021L00312:257,
        F2021L00312:260 ;
    dct:isReferencedBy F2021L00312: ;
    rdfs:comment "Chapter 11 Miscellaneous - Abrievated Graph Key: C241"@en-AU ;
    skos:broader F2021L00312:242,
        F2021L00312:244,
        F2021L00312:254,
        F2021L00312:257,
        F2021L00312:260 ;
    skos:definition "Chapter 11 Miscellaneous"@en-AU ;
    skos:prefLabel "Chapter C241"@en-AU ;
    dcat:accessURL <https://www.legislation.gov.au/F2021L00312/asmade/2021-03-24/text/original/epub/OEBPS/document_1/document_1.html#_Toc65843525> ;
    dcat:landingPage "https://www.legislation.gov.au/F2021L00312/asmade/2021-03-24/text/original/epub/OEBPS/document_1/document_1.html#_Toc65843525"^^xsd:anyURI ;
    dcat:theme legcons:Chapter .

F2021L00312:34 a legcons:Chapter,
        owl:Class,
        dcat:Resource ;
    rdfs:label "Chapter - C34 Chapter 4 Registered establishments"@en-AU ;
    dct:hasPart F2021L00312:35,
        F2021L00312:49,
        F2021L00312:53,
        F2021L00312:56,
        F2021L00312:59 ;
    dct:isReferencedBy F2021L00312: ;
    rdfs:comment "Chapter 4 Registered establishments - Abrievated Graph Key: C34"@en-AU ;
    skos:broader F2021L00312:35,
        F2021L00312:49,
        F2021L00312:53,
        F2021L00312:56,
        F2021L00312:59 ;
    skos:definition "Chapter 4 Registered establishments"@en-AU ;
    skos:prefLabel "Chapter C34"@en-AU ;
    dcat:accessURL <https://www.legislation.gov.au/F2021L00312/asmade/2021-03-24/text/original/epub/OEBPS/document_1/document_1.html#_Toc65843318> ;
    dcat:landingPage "https://www.legislation.gov.au/F2021L00312/asmade/2021-03-24/text/original/epub/OEBPS/document_1/document_1.html#_Toc65843318"^^xsd:anyURI ;
    dcat:theme legcons:Chapter .

F2021L00312:63 a legcons:Chapter,
        owl:Class,
        dcat:Resource ;
    rdfs:label "Chapter - C63 Chapter 5 Approved arrangements"@en-AU ;
    dct:hasPart F2021L00312:117,
        F2021L00312:119,
        F2021L00312:125,
        F2021L00312:64,
        F2021L00312:70 ;
    dct:isReferencedBy F2021L00312: ;
    rdfs:comment "Chapter 5 Approved arrangements - Abrievated Graph Key: C63"@en-AU ;
    skos:broader F2021L00312:117,
        F2021L00312:119,
        F2021L00312:125,
        F2021L00312:64,
        F2021L00312:70 ;
    skos:definition "Chapter 5 Approved arrangements"@en-AU ;
    skos:prefLabel "Chapter C63"@en-AU ;
    dcat:accessURL <https://www.legislation.gov.au/F2021L00312/asmade/2021-03-24/text/original/epub/OEBPS/document_1/document_1.html#_Toc65843347> ;
    dcat:landingPage "https://www.legislation.gov.au/F2021L00312/asmade/2021-03-24/text/original/epub/OEBPS/document_1/document_1.html#_Toc65843347"^^xsd:anyURI ;
    dcat:theme legcons:Chapter .

F2021L00312:97 a legcons:Division,
        owl:Class,
        dcat:Resource ;
    rdfs:label "Division - D97 Division 5 Trade descriptions"@en-AU ;
    dct:hasPart F2021L00312:100,
        F2021L00312:101,
        F2021L00312:98,
        F2021L00312:99 ;
    dct:isPartOf F2021L00312:70 ;
    dct:isReferencedBy F2021L00312: ;
    rdfs:comment "Division 5 Trade descriptions - Abrievated Graph Key: D97"@en-AU ;
    skos:broader F2021L00312:100,
        F2021L00312:101,
        F2021L00312:98,
        F2021L00312:99 ;
    skos:definition "Division 5 Trade descriptions"@en-AU ;
    skos:narrower F2021L00312:70 ;
    skos:prefLabel "Division D97"@en-AU ;
    dcat:accessURL <https://www.legislation.gov.au/F2021L00312/asmade/2021-03-24/text/original/epub/OEBPS/document_1/document_1.html#_Toc65843381> ;
    dcat:landingPage "https://www.legislation.gov.au/F2021L00312/asmade/2021-03-24/text/original/epub/OEBPS/document_1/document_1.html#_Toc65843381"^^xsd:anyURI ;
    dcat:theme legcons:Division .

F2021L00312:111 a legcons:Division,
        owl:Class,
        dcat:Resource ;
    rdfs:label "Division - D111 Division 9 Management practicesexport operations"@en-AU ;
    dct:hasPart F2021L00312:112,
        F2021L00312:113,
        F2021L00312:114,
        F2021L00312:115,
        F2021L00312:116 ;
    dct:isPartOf F2021L00312:70 ;
    dct:isReferencedBy F2021L00312: ;
    rdfs:comment "Division 9 Management practicesexport operations - Abrievated Graph Key: D111"@en-AU ;
    skos:broader F2021L00312:112,
        F2021L00312:113,
        F2021L00312:114,
        F2021L00312:115,
        F2021L00312:116 ;
    skos:definition "Division 9 Management practicesexport operations"@en-AU ;
    skos:narrower F2021L00312:70 ;
    skos:prefLabel "Division D111"@en-AU ;
    dcat:accessURL <https://www.legislation.gov.au/F2021L00312/asmade/2021-03-24/text/original/epub/OEBPS/document_1/document_1.html#_Toc65843395> ;
    dcat:landingPage "https://www.legislation.gov.au/F2021L00312/asmade/2021-03-24/text/original/epub/OEBPS/document_1/document_1.html#_Toc65843395"^^xsd:anyURI ;
    dcat:theme legcons:Division .

F2021L00312:64 a legcons:Part,
        owl:Class,
        dcat:Resource ;
    rdfs:label "Part - P64 Part 1 Requirements for approval"@en-AU ;
    dct:hasPart F2021L00312:65,
        F2021L00312:66,
        F2021L00312:67,
        F2021L00312:68,
        F2021L00312:69 ;
    dct:isPartOf F2021L00312:63 ;
    dct:isReferencedBy F2021L00312: ;
    rdfs:comment "Part 1 Requirements for approval - Abrievated Graph Key: P64"@en-AU ;
    skos:broader F2021L00312:65,
        F2021L00312:66,
        F2021L00312:67,
        F2021L00312:68,
        F2021L00312:69 ;
    skos:definition "Part 1 Requirements for approval"@en-AU ;
    skos:narrower F2021L00312:63 ;
    skos:prefLabel "Part P64"@en-AU ;
    dcat:accessURL <https://www.legislation.gov.au/F2021L00312/asmade/2021-03-24/text/original/epub/OEBPS/document_1/document_1.html#_Toc65843348> ;
    dcat:landingPage "https://www.legislation.gov.au/F2021L00312/asmade/2021-03-24/text/original/epub/OEBPS/document_1/document_1.html#_Toc65843348"^^xsd:anyURI ;
    dcat:theme legcons:Part .

F2021L00312:75 a legcons:Division,
        owl:Class,
        dcat:Resource ;
    rdfs:label "Division - D75 Division 3 Operational hygiene"@en-AU ;
    dct:hasPart F2021L00312:76,
        F2021L00312:77,
        F2021L00312:78,
        F2021L00312:79,
        F2021L00312:80 ;
    dct:isPartOf F2021L00312:70 ;
    dct:isReferencedBy F2021L00312: ;
    rdfs:comment "Division 3 Operational hygiene - Abrievated Graph Key: D75"@en-AU ;
    skos:broader F2021L00312:76,
        F2021L00312:77,
        F2021L00312:78,
        F2021L00312:79,
        F2021L00312:80 ;
    skos:definition "Division 3 Operational hygiene"@en-AU ;
    skos:narrower F2021L00312:70 ;
    skos:prefLabel "Division D75"@en-AU ;
    dcat:accessURL <https://www.legislation.gov.au/F2021L00312/asmade/2021-03-24/text/original/epub/OEBPS/document_1/document_1.html#_Toc65843359> ;
    dcat:landingPage "https://www.legislation.gov.au/F2021L00312/asmade/2021-03-24/text/original/epub/OEBPS/document_1/document_1.html#_Toc65843359"^^xsd:anyURI ;
    dcat:theme legcons:Division .

F2021L00312:177 a legcons:Division,
        owl:Class,
        dcat:Resource ;
    rdfs:label "Division - D177 Division 4 Official marking devices"@en-AU ;
    dct:hasPart F2021L00312:178,
        F2021L00312:179,
        F2021L00312:180,
        F2021L00312:181,
        F2021L00312:182,
        F2021L00312:183 ;
    dct:isPartOf F2021L00312:149 ;
    dct:isReferencedBy F2021L00312: ;
    rdfs:comment "Division 4 Official marking devices - Abrievated Graph Key: D177"@en-AU ;
    skos:broader F2021L00312:178,
        F2021L00312:179,
        F2021L00312:180,
        F2021L00312:181,
        F2021L00312:182,
        F2021L00312:183 ;
    skos:definition "Division 4 Official marking devices"@en-AU ;
    skos:narrower F2021L00312:149 ;
    skos:prefLabel "Division D177"@en-AU ;
    dcat:accessURL <https://www.legislation.gov.au/F2021L00312/asmade/2021-03-24/text/original/epub/OEBPS/document_1/document_1.html#_Toc65843461> ;
    dcat:landingPage "https://www.legislation.gov.au/F2021L00312/asmade/2021-03-24/text/original/epub/OEBPS/document_1/document_1.html#_Toc65843461"^^xsd:anyURI ;
    dcat:theme legcons:Division .

F2021L00312:1 a legcons:Chapter,
        owl:Class,
        dcat:Resource ;
    rdfs:label "Chapter - C1 Chapter 1 Preliminary"@en-AU ;
    dct:hasPart F2021L00312:2,
        F2021L00312:3,
        F2021L00312:4,
        F2021L00312:5,
        F2021L00312:6,
        F2021L00312:7,
        F2021L00312:8,
        F2021L00312:9 ;
    dct:isReferencedBy F2021L00312: ;
    rdfs:comment "Chapter 1 Preliminary - Abrievated Graph Key: C1"@en-AU ;
    skos:broader F2021L00312:2,
        F2021L00312:3,
        F2021L00312:4,
        F2021L00312:5,
        F2021L00312:6,
        F2021L00312:7,
        F2021L00312:8,
        F2021L00312:9 ;
    skos:definition "Chapter 1 Preliminary"@en-AU ;
    skos:prefLabel "Chapter C1"@en-AU ;
    dcat:accessURL <https://www.legislation.gov.au/F2021L00312/asmade/2021-03-24/text/original/epub/OEBPS/document_1/document_1.html#_Toc65843285> ;
    dcat:landingPage "https://www.legislation.gov.au/F2021L00312/asmade/2021-03-24/text/original/epub/OEBPS/document_1/document_1.html#_Toc65843285"^^xsd:anyURI ;
    dcat:theme legcons:Chapter .

F2021L00312:150 a legcons:Division,
        owl:Class,
        dcat:Resource ;
    rdfs:label "Division - D150 Division 1 Marks that are official marks"@en-AU ;
    dct:hasPart F2021L00312:151,
        F2021L00312:152,
        F2021L00312:153,
        F2021L00312:154,
        F2021L00312:155,
        F2021L00312:156,
        F2021L00312:157,
        F2021L00312:158,
        F2021L00312:159 ;
    dct:isPartOf F2021L00312:149 ;
    dct:isReferencedBy F2021L00312: ;
    rdfs:comment "Division 1 Marks that are official marks - Abrievated Graph Key: D150"@en-AU ;
    skos:broader F2021L00312:151,
        F2021L00312:152,
        F2021L00312:153,
        F2021L00312:154,
        F2021L00312:155,
        F2021L00312:156,
        F2021L00312:157,
        F2021L00312:158,
        F2021L00312:159 ;
    skos:definition "Division 1 Marks that are official marks"@en-AU ;
    skos:narrower F2021L00312:149 ;
    skos:prefLabel "Division D150"@en-AU ;
    dcat:accessURL <https://www.legislation.gov.au/F2021L00312/asmade/2021-03-24/text/original/epub/OEBPS/document_1/document_1.html#_Toc65843434> ;
    dcat:landingPage "https://www.legislation.gov.au/F2021L00312/asmade/2021-03-24/text/original/epub/OEBPS/document_1/document_1.html#_Toc65843434"^^xsd:anyURI ;
    dcat:theme legcons:Division .

F2021L00312:244 a legcons:Part,
        owl:Class,
        dcat:Resource ;
    rdfs:label "Part - P244 Part 2 Records"@en-AU ;
    dct:hasPart F2021L00312:245,
        F2021L00312:246,
        F2021L00312:247,
        F2021L00312:248,
        F2021L00312:249,
        F2021L00312:250,
        F2021L00312:251,
        F2021L00312:252,
        F2021L00312:253 ;
    dct:isPartOf F2021L00312:241 ;
    dct:isReferencedBy F2021L00312: ;
    rdfs:comment "Part 2 Records - Abrievated Graph Key: P244"@en-AU ;
    skos:broader F2021L00312:245,
        F2021L00312:246,
        F2021L00312:247,
        F2021L00312:248,
        F2021L00312:249,
        F2021L00312:250,
        F2021L00312:251,
        F2021L00312:252,
        F2021L00312:253 ;
    skos:definition "Part 2 Records"@en-AU ;
    skos:narrower F2021L00312:241 ;
    skos:prefLabel "Part P244"@en-AU ;
    dcat:accessURL <https://www.legislation.gov.au/F2021L00312/asmade/2021-03-24/text/original/epub/OEBPS/document_1/document_1.html#_Toc65843528> ;
    dcat:landingPage "https://www.legislation.gov.au/F2021L00312/asmade/2021-03-24/text/original/epub/OEBPS/document_1/document_1.html#_Toc65843528"^^xsd:anyURI ;
    dcat:theme legcons:Part .

F2021L00312:36 a legcons:Division,
        owl:Class,
        dcat:Resource ;
    rdfs:label "Division - D36 Division 1 Requirements relating to construction equipment and facilities"@en-AU ;
    dct:hasPart F2021L00312:37,
        F2021L00312:38,
        F2021L00312:39,
        F2021L00312:40,
        F2021L00312:41,
        F2021L00312:42,
        F2021L00312:43,
        F2021L00312:44,
        F2021L00312:45 ;
    dct:isPartOf F2021L00312:35 ;
    dct:isReferencedBy F2021L00312: ;
    rdfs:comment "Division 1 Requirements relating to construction equipment and facilities - Abrievated Graph Key: D36"@en-AU ;
    skos:broader F2021L00312:37,
        F2021L00312:38,
        F2021L00312:39,
        F2021L00312:40,
        F2021L00312:41,
        F2021L00312:42,
        F2021L00312:43,
        F2021L00312:44,
        F2021L00312:45 ;
    skos:definition "Division 1 Requirements relating to construction equipment and facilities"@en-AU ;
    skos:narrower F2021L00312:35 ;
    skos:prefLabel "Division D36"@en-AU ;
    dcat:accessURL <https://www.legislation.gov.au/F2021L00312/asmade/2021-03-24/text/original/epub/OEBPS/document_1/document_1.html#_Toc65843320> ;
    dcat:landingPage "https://www.legislation.gov.au/F2021L00312/asmade/2021-03-24/text/original/epub/OEBPS/document_1/document_1.html#_Toc65843320"^^xsd:anyURI ;
    dcat:theme legcons:Division .

F2021L00312:70 a legcons:Part,
        owl:Class,
        dcat:Resource ;
    rdfs:label "Part - P70 Part 2 Conditions of approved arrangement"@en-AU ;
    dct:hasPart F2021L00312:102,
        F2021L00312:104,
        F2021L00312:108,
        F2021L00312:111,
        F2021L00312:71,
        F2021L00312:73,
        F2021L00312:75,
        F2021L00312:81,
        F2021L00312:97 ;
    dct:isPartOf F2021L00312:63 ;
    dct:isReferencedBy F2021L00312: ;
    rdfs:comment "Part 2 Conditions of approved arrangement - Abrievated Graph Key: P70"@en-AU ;
    skos:broader F2021L00312:102,
        F2021L00312:104,
        F2021L00312:108,
        F2021L00312:111,
        F2021L00312:71,
        F2021L00312:73,
        F2021L00312:75,
        F2021L00312:81,
        F2021L00312:97 ;
    skos:definition "Part 2 Conditions of approved arrangement"@en-AU ;
    skos:narrower F2021L00312:63 ;
    skos:prefLabel "Part P70"@en-AU ;
    dcat:accessURL <https://www.legislation.gov.au/F2021L00312/asmade/2021-03-24/text/original/epub/OEBPS/document_1/document_1.html#_Toc65843354> ;
    dcat:landingPage "https://www.legislation.gov.au/F2021L00312/asmade/2021-03-24/text/original/epub/OEBPS/document_1/document_1.html#_Toc65843354"^^xsd:anyURI ;
    dcat:theme legcons:Part .

F2021L00312:194 a legcons:Division,
        owl:Class,
        dcat:Resource ;
    rdfs:label "Division - D194 Division 3 Approved auditors"@en-AU ;
    dct:hasPart F2021L00312:195,
        F2021L00312:196,
        F2021L00312:197,
        F2021L00312:198,
        F2021L00312:199,
        F2021L00312:200,
        F2021L00312:201,
        F2021L00312:202,
        F2021L00312:203,
        F2021L00312:204,
        F2021L00312:205 ;
    dct:isPartOf F2021L00312:185 ;
    dct:isReferencedBy F2021L00312: ;
    rdfs:comment "Division 3 Approved auditors - Abrievated Graph Key: D194"@en-AU ;
    skos:broader F2021L00312:195,
        F2021L00312:196,
        F2021L00312:197,
        F2021L00312:198,
        F2021L00312:199,
        F2021L00312:200,
        F2021L00312:201,
        F2021L00312:202,
        F2021L00312:203,
        F2021L00312:204,
        F2021L00312:205 ;
    skos:definition "Division 3 Approved auditors"@en-AU ;
    skos:narrower F2021L00312:185 ;
    skos:prefLabel "Division D194"@en-AU ;
    dcat:accessURL <https://www.legislation.gov.au/F2021L00312/asmade/2021-03-24/text/original/epub/OEBPS/document_1/document_1.html#_Toc65843478> ;
    dcat:landingPage "https://www.legislation.gov.au/F2021L00312/asmade/2021-03-24/text/original/epub/OEBPS/document_1/document_1.html#_Toc65843478"^^xsd:anyURI ;
    dcat:theme legcons:Division .

F2021L00312:212 a legcons:Division,
        owl:Class,
        dcat:Resource ;
    rdfs:label "Division - D212 Division 3 Approved assessors"@en-AU ;
    dct:hasPart F2021L00312:213,
        F2021L00312:214,
        F2021L00312:215,
        F2021L00312:216,
        F2021L00312:217,
        F2021L00312:218,
        F2021L00312:219,
        F2021L00312:220,
        F2021L00312:221,
        F2021L00312:222,
        F2021L00312:223 ;
    dct:isPartOf F2021L00312:206 ;
    dct:isReferencedBy F2021L00312: ;
    rdfs:comment "Division 3 Approved assessors - Abrievated Graph Key: D212"@en-AU ;
    skos:broader F2021L00312:213,
        F2021L00312:214,
        F2021L00312:215,
        F2021L00312:216,
        F2021L00312:217,
        F2021L00312:218,
        F2021L00312:219,
        F2021L00312:220,
        F2021L00312:221,
        F2021L00312:222,
        F2021L00312:223 ;
    skos:definition "Division 3 Approved assessors"@en-AU ;
    skos:narrower F2021L00312:206 ;
    skos:prefLabel "Division D212"@en-AU ;
    dcat:accessURL <https://www.legislation.gov.au/F2021L00312/asmade/2021-03-24/text/original/epub/OEBPS/document_1/document_1.html#_Toc65843496> ;
    dcat:landingPage "https://www.legislation.gov.au/F2021L00312/asmade/2021-03-24/text/original/epub/OEBPS/document_1/document_1.html#_Toc65843496"^^xsd:anyURI ;
    dcat:theme legcons:Division .

F2021L00312:160 a legcons:Division,
        owl:Class,
        dcat:Resource ;
    rdfs:label "Division - D160 Division 2 General rules relating to official marks"@en-AU ;
    dct:hasPart F2021L00312:161,
        F2021L00312:162,
        F2021L00312:163,
        F2021L00312:164,
        F2021L00312:165,
        F2021L00312:166,
        F2021L00312:167,
        F2021L00312:168,
        F2021L00312:169,
        F2021L00312:170,
        F2021L00312:171,
        F2021L00312:172 ;
    dct:isPartOf F2021L00312:149 ;
    dct:isReferencedBy F2021L00312: ;
    rdfs:comment "Division 2 General rules relating to official marks - Abrievated Graph Key: D160"@en-AU ;
    skos:broader F2021L00312:161,
        F2021L00312:162,
        F2021L00312:163,
        F2021L00312:164,
        F2021L00312:165,
        F2021L00312:166,
        F2021L00312:167,
        F2021L00312:168,
        F2021L00312:169,
        F2021L00312:170,
        F2021L00312:171,
        F2021L00312:172 ;
    skos:definition "Division 2 General rules relating to official marks"@en-AU ;
    skos:narrower F2021L00312:149 ;
    skos:prefLabel "Division D160"@en-AU ;
    dcat:accessURL <https://www.legislation.gov.au/F2021L00312/asmade/2021-03-24/text/original/epub/OEBPS/document_1/document_1.html#_Toc65843444> ;
    dcat:landingPage "https://www.legislation.gov.au/F2021L00312/asmade/2021-03-24/text/original/epub/OEBPS/document_1/document_1.html#_Toc65843444"^^xsd:anyURI ;
    dcat:theme legcons:Division .

F2021L00312:81 a legcons:Division,
        owl:Class,
        dcat:Resource ;
    rdfs:label "Division - D81 Division 4 Preparation and transport"@en-AU ;
    dct:hasPart F2021L00312:82,
        F2021L00312:83,
        F2021L00312:84,
        F2021L00312:85,
        F2021L00312:86,
        F2021L00312:87,
        F2021L00312:88,
        F2021L00312:89,
        F2021L00312:90,
        F2021L00312:91,
        F2021L00312:92,
        F2021L00312:93,
        F2021L00312:94,
        F2021L00312:95,
        F2021L00312:96 ;
    dct:isPartOf F2021L00312:70 ;
    dct:isReferencedBy F2021L00312: ;
    rdfs:comment "Division 4 Preparation and transport - Abrievated Graph Key: D81"@en-AU ;
    skos:broader F2021L00312:82,
        F2021L00312:83,
        F2021L00312:84,
        F2021L00312:85,
        F2021L00312:86,
        F2021L00312:87,
        F2021L00312:88,
        F2021L00312:89,
        F2021L00312:90,
        F2021L00312:91,
        F2021L00312:92,
        F2021L00312:93,
        F2021L00312:94,
        F2021L00312:95,
        F2021L00312:96 ;
    skos:definition "Division 4 Preparation and transport"@en-AU ;
    skos:narrower F2021L00312:70 ;
    skos:prefLabel "Division D81"@en-AU ;
    dcat:accessURL <https://www.legislation.gov.au/F2021L00312/asmade/2021-03-24/text/original/epub/OEBPS/document_1/document_1.html#_Toc65843365> ;
    dcat:landingPage "https://www.legislation.gov.au/F2021L00312/asmade/2021-03-24/text/original/epub/OEBPS/document_1/document_1.html#_Toc65843365"^^xsd:anyURI ;
    dcat:theme legcons:Division .

F2021L00312:10 a legcons:Chapter,
        owl:Class,
        dcat:Resource ;
    rdfs:label "Chapter - C10 Chapter 2 Exporting goods"@en-AU ;
    dct:hasPart F2021L00312:11,
        F2021L00312:18,
        F2021L00312:19,
        F2021L00312:20,
        F2021L00312:21,
        F2021L00312:22,
        F2021L00312:23,
        F2021L00312:24,
        F2021L00312:25,
        F2021L00312:26,
        F2021L00312:27,
        F2021L00312:28,
        F2021L00312:29,
        F2021L00312:30,
        F2021L00312:31,
        F2021L00312:32,
        F2021L00312:33 ;
    dct:isReferencedBy F2021L00312: ;
    rdfs:comment "Chapter 2 Exporting goods - Abrievated Graph Key: C10"@en-AU ;
    skos:broader F2021L00312:11,
        F2021L00312:18,
        F2021L00312:19,
        F2021L00312:20,
        F2021L00312:21,
        F2021L00312:22,
        F2021L00312:23,
        F2021L00312:24,
        F2021L00312:25,
        F2021L00312:26,
        F2021L00312:27,
        F2021L00312:28,
        F2021L00312:29,
        F2021L00312:30,
        F2021L00312:31,
        F2021L00312:32,
        F2021L00312:33 ;
    skos:definition "Chapter 2 Exporting goods"@en-AU ;
    skos:prefLabel "Chapter C10"@en-AU ;
    dcat:accessURL <https://www.legislation.gov.au/F2021L00312/asmade/2021-03-24/text/original/epub/OEBPS/document_1/document_1.html#_Toc65843294> ;
    dcat:landingPage "https://www.legislation.gov.au/F2021L00312/asmade/2021-03-24/text/original/epub/OEBPS/document_1/document_1.html#_Toc65843294"^^xsd:anyURI ;
    dcat:theme legcons:Chapter .

F2021L00312: a owl:Class,
        dcat:Dataset,
        dcat:Resource ;
    rdfs:label "Export Control (Eggs and Egg Products) Rules 2021" ;
    dct:Jurisdiction " Department of Agriculture, Fisheries and Forestry "@en-AU ;
    dct:created "2024-08-30T15:12:38.307424"^^xsd:dateTime ;
    dct:creator "https://orcid.org/0009-0007-8434-7325"^^xsd:anyURI ;
    dct:date "2021-03-24T00:00:00+11:00"^^xsd:dateTime ;
    dct:description "Export Control (Eggs and Egg Products) Rules 2021"@en-AU ;
    dct:identifier "https://www.legislation.gov.au/F2021L00312/asmade"^^xsd:anyURI ;
    dct:license <https://creativecommons.org/licenses/by-sa/4.0/> ;
    dct:source "scheme=AGLSTERMS.AglsAgent; corporateName=Office Parliamentary Counsel; address=Locked Bag 30 Kingston ACT 2604; contact=+61 2 6120 1400"@en-AU ;
    dct:subject "Export Control (Eggs and Egg Products) Rules 2021"@en-AU ;
    dct:title "Export Control (Eggs and Egg Products) Rules 2021"@en-AU ;
    owl:imports legcons: ;
    dcat:theme legcons:Chapter,
        legcons:Division,
        legcons:Item,
        legcons:Part ;
    schema:identifier "F2021L00312" ;
    schema:status "In force" ;
    schema:version "F2021L00312" .

