@prefix F2021L00317: <http://example.org/au/leg/dataset/F2021L00317/> .
@prefix dcat: <http://www.w3.org/ns/dcat#> .
@prefix dct: <http://purl.org/dc/terms/> .
@prefix legcons: <http://example.org/au/leg/concepts/> .
@prefix owl: <http://www.w3.org/2002/07/owl#> .
@prefix rdfs: <http://www.w3.org/2000/01/rdf-schema#> .
@prefix schema: <https://schema.org/> .
@prefix skos: <http://www.w3.org/2004/02/skos/core#> .
@prefix xsd: <http://www.w3.org/2001/XMLSchema#> .

F2021L00317:10 a legcons:Item,
        owl:Class,
        dcat:Resource ;
    rdfs:label "Item - I10 1 7  Meaning of loaded for export"@en-AU ;
    dct:isPartOf F2021L00317:1 ;
    dct:isReferencedBy F2021L00317: ;
    rdfs:comment "1 7  Meaning of loaded for export - Abrievated Graph Key: I10"@en-AU ;
    skos:definition "1 7  Meaning of loaded for export"@en-AU ;
    skos:narrower F2021L00317:1 ;
    skos:prefLabel "Item I10"@en-AU ;
    dcat:accessURL <https://www.legislation.gov.au/F2021L00317/asmade/2021-03-24/text/original/epub/OEBPS/document_1/document_1.html#_Toc66194767> ;
    dcat:landingPage "https://www.legislation.gov.au/F2021L00317/asmade/2021-03-24/text/original/epub/OEBPS/document_1/document_1.html#_Toc66194767"^^xsd:anyURI ;
    dcat:theme legcons:Item .

F2021L00317:100 a legcons:Item,
        owl:Class,
        dcat:Resource ;
    rdfs:label "Item - I100 5 26  Transport"@en-AU ;
    dct:isPartOf F2021L00317:88 ;
    dct:isReferencedBy F2021L00317: ;
    rdfs:comment "5 26  Transport - Abrievated Graph Key: I100"@en-AU ;
    skos:definition "5 26  Transport"@en-AU ;
    skos:narrower F2021L00317:88 ;
    skos:prefLabel "Item I100"@en-AU ;
    dcat:accessURL <https://www.legislation.gov.au/F2021L00317/asmade/2021-03-24/text/original/epub/OEBPS/document_1/document_1.html#_Toc66194857> ;
    dcat:landingPage "https://www.legislation.gov.au/F2021L00317/asmade/2021-03-24/text/original/epub/OEBPS/document_1/document_1.html#_Toc66194857"^^xsd:anyURI ;
    dcat:theme legcons:Item .

F2021L00317:101 a legcons:Item,
        owl:Class,
        dcat:Resource ;
    rdfs:label "Item - I101 5 27  Identification as not for export as foodfitness for human consumption etc"@en-AU ;
    dct:isPartOf F2021L00317:88 ;
    dct:isReferencedBy F2021L00317: ;
    rdfs:comment "5 27  Identification as not for export as foodfitness for human consumption etc - Abrievated Graph Key: I101"@en-AU ;
    skos:definition "5 27  Identification as not for export as foodfitness for human consumption etc"@en-AU ;
    skos:narrower F2021L00317:88 ;
    skos:prefLabel "Item I101"@en-AU ;
    dcat:accessURL <https://www.legislation.gov.au/F2021L00317/asmade/2021-03-24/text/original/epub/OEBPS/document_1/document_1.html#_Toc66194858> ;
    dcat:landingPage "https://www.legislation.gov.au/F2021L00317/asmade/2021-03-24/text/original/epub/OEBPS/document_1/document_1.html#_Toc66194858"^^xsd:anyURI ;
    dcat:theme legcons:Item .

F2021L00317:102 a legcons:Item,
        owl:Class,
        dcat:Resource ;
    rdfs:label "Item - I102 5 28  Product standardsgeneral"@en-AU ;
    dct:isPartOf F2021L00317:88 ;
    dct:isReferencedBy F2021L00317: ;
    rdfs:comment "5 28  Product standardsgeneral - Abrievated Graph Key: I102"@en-AU ;
    skos:definition "5 28  Product standardsgeneral"@en-AU ;
    skos:narrower F2021L00317:88 ;
    skos:prefLabel "Item I102"@en-AU ;
    dcat:accessURL <https://www.legislation.gov.au/F2021L00317/asmade/2021-03-24/text/original/epub/OEBPS/document_1/document_1.html#_Toc66194859> ;
    dcat:landingPage "https://www.legislation.gov.au/F2021L00317/asmade/2021-03-24/text/original/epub/OEBPS/document_1/document_1.html#_Toc66194859"^^xsd:anyURI ;
    dcat:theme legcons:Item .

F2021L00317:104 a legcons:Item,
        owl:Class,
        dcat:Resource ;
    rdfs:label "Item - I104 5 29  Harvesting shellfish"@en-AU ;
    dct:isPartOf F2021L00317:103 ;
    dct:isReferencedBy F2021L00317: ;
    rdfs:comment "5 29  Harvesting shellfish - Abrievated Graph Key: I104"@en-AU ;
    skos:definition "5 29  Harvesting shellfish"@en-AU ;
    skos:narrower F2021L00317:103 ;
    skos:prefLabel "Item I104"@en-AU ;
    dcat:accessURL <https://www.legislation.gov.au/F2021L00317/asmade/2021-03-24/text/original/epub/OEBPS/document_1/document_1.html#_Toc66194861> ;
    dcat:landingPage "https://www.legislation.gov.au/F2021L00317/asmade/2021-03-24/text/original/epub/OEBPS/document_1/document_1.html#_Toc66194861"^^xsd:anyURI ;
    dcat:theme legcons:Item .

F2021L00317:105 a legcons:Item,
        owl:Class,
        dcat:Resource ;
    rdfs:label "Item - I105 5 30  Handling shellfish"@en-AU ;
    dct:isPartOf F2021L00317:103 ;
    dct:isReferencedBy F2021L00317: ;
    rdfs:comment "5 30  Handling shellfish - Abrievated Graph Key: I105"@en-AU ;
    skos:definition "5 30  Handling shellfish"@en-AU ;
    skos:narrower F2021L00317:103 ;
    skos:prefLabel "Item I105"@en-AU ;
    dcat:accessURL <https://www.legislation.gov.au/F2021L00317/asmade/2021-03-24/text/original/epub/OEBPS/document_1/document_1.html#_Toc66194862> ;
    dcat:landingPage "https://www.legislation.gov.au/F2021L00317/asmade/2021-03-24/text/original/epub/OEBPS/document_1/document_1.html#_Toc66194862"^^xsd:anyURI ;
    dcat:theme legcons:Item .

F2021L00317:106 a legcons:Item,
        owl:Class,
        dcat:Resource ;
    rdfs:label "Item - I106 5 31  Depuration of shellfish"@en-AU ;
    dct:isPartOf F2021L00317:103 ;
    dct:isReferencedBy F2021L00317: ;
    rdfs:comment "5 31  Depuration of shellfish - Abrievated Graph Key: I106"@en-AU ;
    skos:definition "5 31  Depuration of shellfish"@en-AU ;
    skos:narrower F2021L00317:103 ;
    skos:prefLabel "Item I106"@en-AU ;
    dcat:accessURL <https://www.legislation.gov.au/F2021L00317/asmade/2021-03-24/text/original/epub/OEBPS/document_1/document_1.html#_Toc66194863> ;
    dcat:landingPage "https://www.legislation.gov.au/F2021L00317/asmade/2021-03-24/text/original/epub/OEBPS/document_1/document_1.html#_Toc66194863"^^xsd:anyURI ;
    dcat:theme legcons:Item .

F2021L00317:108 a legcons:Item,
        owl:Class,
        dcat:Resource ;
    rdfs:label "Item - I108 5 32  Handling crocodiles and crocodile meat"@en-AU ;
    dct:isPartOf F2021L00317:107 ;
    dct:isReferencedBy F2021L00317: ;
    rdfs:comment "5 32  Handling crocodiles and crocodile meat - Abrievated Graph Key: I108"@en-AU ;
    skos:definition "5 32  Handling crocodiles and crocodile meat"@en-AU ;
    skos:narrower F2021L00317:107 ;
    skos:prefLabel "Item I108"@en-AU ;
    dcat:accessURL <https://www.legislation.gov.au/F2021L00317/asmade/2021-03-24/text/original/epub/OEBPS/document_1/document_1.html#_Toc66194865> ;
    dcat:landingPage "https://www.legislation.gov.au/F2021L00317/asmade/2021-03-24/text/original/epub/OEBPS/document_1/document_1.html#_Toc66194865"^^xsd:anyURI ;
    dcat:theme legcons:Item .

F2021L00317:109 a legcons:Item,
        owl:Class,
        dcat:Resource ;
    rdfs:label "Item - I109 5 33  Post mortem controls for crocodile carcases"@en-AU ;
    dct:isPartOf F2021L00317:107 ;
    dct:isReferencedBy F2021L00317: ;
    rdfs:comment "5 33  Post mortem controls for crocodile carcases - Abrievated Graph Key: I109"@en-AU ;
    skos:definition "5 33  Post mortem controls for crocodile carcases"@en-AU ;
    skos:narrower F2021L00317:107 ;
    skos:prefLabel "Item I109"@en-AU ;
    dcat:accessURL <https://www.legislation.gov.au/F2021L00317/asmade/2021-03-24/text/original/epub/OEBPS/document_1/document_1.html#_Toc66194866> ;
    dcat:landingPage "https://www.legislation.gov.au/F2021L00317/asmade/2021-03-24/text/original/epub/OEBPS/document_1/document_1.html#_Toc66194866"^^xsd:anyURI ;
    dcat:theme legcons:Item .

F2021L00317:110 a legcons:Item,
        owl:Class,
        dcat:Resource ;
    rdfs:label "Item - I110 5 34  Temperature controls for preparation of crocodile meat products"@en-AU ;
    dct:isPartOf F2021L00317:107 ;
    dct:isReferencedBy F2021L00317: ;
    rdfs:comment "5 34  Temperature controls for preparation of crocodile meat products - Abrievated Graph Key: I110"@en-AU ;
    skos:definition "5 34  Temperature controls for preparation of crocodile meat products"@en-AU ;
    skos:narrower F2021L00317:107 ;
    skos:prefLabel "Item I110"@en-AU ;
    dcat:accessURL <https://www.legislation.gov.au/F2021L00317/asmade/2021-03-24/text/original/epub/OEBPS/document_1/document_1.html#_Toc66194867> ;
    dcat:landingPage "https://www.legislation.gov.au/F2021L00317/asmade/2021-03-24/text/original/epub/OEBPS/document_1/document_1.html#_Toc66194867"^^xsd:anyURI ;
    dcat:theme legcons:Item .

F2021L00317:111 a legcons:Division,
        owl:Class,
        dcat:Resource ;
    rdfs:label "Division - D111 Division 5 Trade descriptions"@en-AU ;
    dct:isPartOf F2021L00317:72 ;
    dct:isReferencedBy F2021L00317: ;
    rdfs:comment "Division 5 Trade descriptions - Abrievated Graph Key: D111"@en-AU ;
    skos:definition "Division 5 Trade descriptions"@en-AU ;
    skos:narrower F2021L00317:72 ;
    skos:prefLabel "Division D111"@en-AU ;
    dcat:accessURL <https://www.legislation.gov.au/F2021L00317/asmade/2021-03-24/text/original/epub/OEBPS/document_1/document_1.html#_Toc66194868> ;
    dcat:landingPage "https://www.legislation.gov.au/F2021L00317/asmade/2021-03-24/text/original/epub/OEBPS/document_1/document_1.html#_Toc66194868"^^xsd:anyURI ;
    dcat:theme legcons:Division .

F2021L00317:112 a legcons:Item,
        owl:Class,
        dcat:Resource ;
    rdfs:label "Item - I112 5 35  Trade description must be applied to prescribed fish and fish products"@en-AU ;
    dct:isPartOf F2021L00317:72 ;
    dct:isReferencedBy F2021L00317: ;
    rdfs:comment "5 35  Trade description must be applied to prescribed fish and fish products - Abrievated Graph Key: I112"@en-AU ;
    skos:definition "5 35  Trade description must be applied to prescribed fish and fish products"@en-AU ;
    skos:narrower F2021L00317:72 ;
    skos:prefLabel "Item I112"@en-AU ;
    dcat:accessURL <https://www.legislation.gov.au/F2021L00317/asmade/2021-03-24/text/original/epub/OEBPS/document_1/document_1.html#_Toc66194869> ;
    dcat:landingPage "https://www.legislation.gov.au/F2021L00317/asmade/2021-03-24/text/original/epub/OEBPS/document_1/document_1.html#_Toc66194869"^^xsd:anyURI ;
    dcat:theme legcons:Item .

F2021L00317:113 a legcons:Item,
        owl:Class,
        dcat:Resource ;
    rdfs:label "Item - I113 5 36  Incomplete trade descriptioncanned fish or fish products"@en-AU ;
    dct:isPartOf F2021L00317:72 ;
    dct:isReferencedBy F2021L00317: ;
    rdfs:comment "5 36  Incomplete trade descriptioncanned fish or fish products - Abrievated Graph Key: I113"@en-AU ;
    skos:definition "5 36  Incomplete trade descriptioncanned fish or fish products"@en-AU ;
    skos:narrower F2021L00317:72 ;
    skos:prefLabel "Item I113"@en-AU ;
    dcat:accessURL <https://www.legislation.gov.au/F2021L00317/asmade/2021-03-24/text/original/epub/OEBPS/document_1/document_1.html#_Toc66194870> ;
    dcat:landingPage "https://www.legislation.gov.au/F2021L00317/asmade/2021-03-24/text/original/epub/OEBPS/document_1/document_1.html#_Toc66194870"^^xsd:anyURI ;
    dcat:theme legcons:Item .

F2021L00317:114 a legcons:Item,
        owl:Class,
        dcat:Resource ;
    rdfs:label "Item - I114 5 37  Labelling and naming of ingredients"@en-AU ;
    dct:isPartOf F2021L00317:72 ;
    dct:isReferencedBy F2021L00317: ;
    rdfs:comment "5 37  Labelling and naming of ingredients - Abrievated Graph Key: I114"@en-AU ;
    skos:definition "5 37  Labelling and naming of ingredients"@en-AU ;
    skos:narrower F2021L00317:72 ;
    skos:prefLabel "Item I114"@en-AU ;
    dcat:accessURL <https://www.legislation.gov.au/F2021L00317/asmade/2021-03-24/text/original/epub/OEBPS/document_1/document_1.html#_Toc66194871> ;
    dcat:landingPage "https://www.legislation.gov.au/F2021L00317/asmade/2021-03-24/text/original/epub/OEBPS/document_1/document_1.html#_Toc66194871"^^xsd:anyURI ;
    dcat:theme legcons:Item .

F2021L00317:115 a legcons:Item,
        owl:Class,
        dcat:Resource ;
    rdfs:label "Item - I115 5 38  Trade descriptions applied to packaging etc"@en-AU ;
    dct:isPartOf F2021L00317:72 ;
    dct:isReferencedBy F2021L00317: ;
    rdfs:comment "5 38  Trade descriptions applied to packaging etc - Abrievated Graph Key: I115"@en-AU ;
    skos:definition "5 38  Trade descriptions applied to packaging etc"@en-AU ;
    skos:narrower F2021L00317:72 ;
    skos:prefLabel "Item I115"@en-AU ;
    dcat:accessURL <https://www.legislation.gov.au/F2021L00317/asmade/2021-03-24/text/original/epub/OEBPS/document_1/document_1.html#_Toc66194872> ;
    dcat:landingPage "https://www.legislation.gov.au/F2021L00317/asmade/2021-03-24/text/original/epub/OEBPS/document_1/document_1.html#_Toc66194872"^^xsd:anyURI ;
    dcat:theme legcons:Item .

F2021L00317:116 a legcons:Division,
        owl:Class,
        dcat:Resource ;
    rdfs:label "Division - D116 Division 6 Official marks"@en-AU ;
    dct:isPartOf F2021L00317:72 ;
    dct:isReferencedBy F2021L00317: ;
    rdfs:comment "Division 6 Official marks - Abrievated Graph Key: D116"@en-AU ;
    skos:definition "Division 6 Official marks"@en-AU ;
    skos:narrower F2021L00317:72 ;
    skos:prefLabel "Division D116"@en-AU ;
    dcat:accessURL <https://www.legislation.gov.au/F2021L00317/asmade/2021-03-24/text/original/epub/OEBPS/document_1/document_1.html#_Toc66194873> ;
    dcat:landingPage "https://www.legislation.gov.au/F2021L00317/asmade/2021-03-24/text/original/epub/OEBPS/document_1/document_1.html#_Toc66194873"^^xsd:anyURI ;
    dcat:theme legcons:Division .

F2021L00317:117 a legcons:Item,
        owl:Class,
        dcat:Resource ;
    rdfs:label "Item - I117 5 39  Alteration of or interference with official mark"@en-AU ;
    dct:isPartOf F2021L00317:72 ;
    dct:isReferencedBy F2021L00317: ;
    rdfs:comment "5 39  Alteration of or interference with official mark - Abrievated Graph Key: I117"@en-AU ;
    skos:definition "5 39  Alteration of or interference with official mark"@en-AU ;
    skos:narrower F2021L00317:72 ;
    skos:prefLabel "Item I117"@en-AU ;
    dcat:accessURL <https://www.legislation.gov.au/F2021L00317/asmade/2021-03-24/text/original/epub/OEBPS/document_1/document_1.html#_Toc66194874> ;
    dcat:landingPage "https://www.legislation.gov.au/F2021L00317/asmade/2021-03-24/text/original/epub/OEBPS/document_1/document_1.html#_Toc66194874"^^xsd:anyURI ;
    dcat:theme legcons:Item .

F2021L00317:118 a legcons:Division,
        owl:Class,
        dcat:Resource ;
    rdfs:label "Division - D118 Division 7 Segregation identification security traceability and integrity"@en-AU ;
    dct:isPartOf F2021L00317:72 ;
    dct:isReferencedBy F2021L00317: ;
    rdfs:comment "Division 7 Segregation identification security traceability and integrity - Abrievated Graph Key: D118"@en-AU ;
    skos:definition "Division 7 Segregation identification security traceability and integrity"@en-AU ;
    skos:narrower F2021L00317:72 ;
    skos:prefLabel "Division D118"@en-AU ;
    dcat:accessURL <https://www.legislation.gov.au/F2021L00317/asmade/2021-03-24/text/original/epub/OEBPS/document_1/document_1.html#_Toc66194875> ;
    dcat:landingPage "https://www.legislation.gov.au/F2021L00317/asmade/2021-03-24/text/original/epub/OEBPS/document_1/document_1.html#_Toc66194875"^^xsd:anyURI ;
    dcat:theme legcons:Division .

F2021L00317:119 a legcons:Item,
        owl:Class,
        dcat:Resource ;
    rdfs:label "Item - I119 5 40  Segregation identification and traceabilitygeneral"@en-AU ;
    dct:isPartOf F2021L00317:72 ;
    dct:isReferencedBy F2021L00317: ;
    rdfs:comment "5 40  Segregation identification and traceabilitygeneral - Abrievated Graph Key: I119"@en-AU ;
    skos:definition "5 40  Segregation identification and traceabilitygeneral"@en-AU ;
    skos:narrower F2021L00317:72 ;
    skos:prefLabel "Item I119"@en-AU ;
    dcat:accessURL <https://www.legislation.gov.au/F2021L00317/asmade/2021-03-24/text/original/epub/OEBPS/document_1/document_1.html#_Toc66194876> ;
    dcat:landingPage "https://www.legislation.gov.au/F2021L00317/asmade/2021-03-24/text/original/epub/OEBPS/document_1/document_1.html#_Toc66194876"^^xsd:anyURI ;
    dcat:theme legcons:Item .

F2021L00317:120 a legcons:Item,
        owl:Class,
        dcat:Resource ;
    rdfs:label "Item - I120 5 41  Establishments where fish or fish products that are not for export etc are prepared"@en-AU ;
    dct:isPartOf F2021L00317:72 ;
    dct:isReferencedBy F2021L00317: ;
    rdfs:comment "5 41  Establishments where fish or fish products that are not for export etc are prepared - Abrievated Graph Key: I120"@en-AU ;
    skos:definition "5 41  Establishments where fish or fish products that are not for export etc are prepared"@en-AU ;
    skos:narrower F2021L00317:72 ;
    skos:prefLabel "Item I120"@en-AU ;
    dcat:accessURL <https://www.legislation.gov.au/F2021L00317/asmade/2021-03-24/text/original/epub/OEBPS/document_1/document_1.html#_Toc66194877> ;
    dcat:landingPage "https://www.legislation.gov.au/F2021L00317/asmade/2021-03-24/text/original/epub/OEBPS/document_1/document_1.html#_Toc66194877"^^xsd:anyURI ;
    dcat:theme legcons:Item .

F2021L00317:121 a legcons:Item,
        owl:Class,
        dcat:Resource ;
    rdfs:label "Item - I121 5 42  Integritygeneral"@en-AU ;
    dct:isPartOf F2021L00317:72 ;
    dct:isReferencedBy F2021L00317: ;
    rdfs:comment "5 42  Integritygeneral - Abrievated Graph Key: I121"@en-AU ;
    skos:definition "5 42  Integritygeneral"@en-AU ;
    skos:narrower F2021L00317:72 ;
    skos:prefLabel "Item I121"@en-AU ;
    dcat:accessURL <https://www.legislation.gov.au/F2021L00317/asmade/2021-03-24/text/original/epub/OEBPS/document_1/document_1.html#_Toc66194878> ;
    dcat:landingPage "https://www.legislation.gov.au/F2021L00317/asmade/2021-03-24/text/original/epub/OEBPS/document_1/document_1.html#_Toc66194878"^^xsd:anyURI ;
    dcat:theme legcons:Item .

F2021L00317:122 a legcons:Item,
        owl:Class,
        dcat:Resource ;
    rdfs:label "Item - I122 5 43  Species identification"@en-AU ;
    dct:isPartOf F2021L00317:72 ;
    dct:isReferencedBy F2021L00317: ;
    rdfs:comment "5 43  Species identification - Abrievated Graph Key: I122"@en-AU ;
    skos:definition "5 43  Species identification"@en-AU ;
    skos:narrower F2021L00317:72 ;
    skos:prefLabel "Item I122"@en-AU ;
    dcat:accessURL <https://www.legislation.gov.au/F2021L00317/asmade/2021-03-24/text/original/epub/OEBPS/document_1/document_1.html#_Toc66194879> ;
    dcat:landingPage "https://www.legislation.gov.au/F2021L00317/asmade/2021-03-24/text/original/epub/OEBPS/document_1/document_1.html#_Toc66194879"^^xsd:anyURI ;
    dcat:theme legcons:Item .

F2021L00317:123 a legcons:Division,
        owl:Class,
        dcat:Resource ;
    rdfs:label "Division - D123 Division 8 Transfers"@en-AU ;
    dct:isPartOf F2021L00317:72 ;
    dct:isReferencedBy F2021L00317: ;
    rdfs:comment "Division 8 Transfers - Abrievated Graph Key: D123"@en-AU ;
    skos:definition "Division 8 Transfers"@en-AU ;
    skos:narrower F2021L00317:72 ;
    skos:prefLabel "Division D123"@en-AU ;
    dcat:accessURL <https://www.legislation.gov.au/F2021L00317/asmade/2021-03-24/text/original/epub/OEBPS/document_1/document_1.html#_Toc66194880> ;
    dcat:landingPage "https://www.legislation.gov.au/F2021L00317/asmade/2021-03-24/text/original/epub/OEBPS/document_1/document_1.html#_Toc66194880"^^xsd:anyURI ;
    dcat:theme legcons:Division .

F2021L00317:124 a legcons:Item,
        owl:Class,
        dcat:Resource ;
    rdfs:label "Item - I124 5 44  Information and declarations relating to transferred prescribed fish or fish products"@en-AU ;
    dct:isPartOf F2021L00317:72 ;
    dct:isReferencedBy F2021L00317: ;
    rdfs:comment "5 44  Information and declarations relating to transferred prescribed fish or fish products - Abrievated Graph Key: I124"@en-AU ;
    skos:definition "5 44  Information and declarations relating to transferred prescribed fish or fish products"@en-AU ;
    skos:narrower F2021L00317:72 ;
    skos:prefLabel "Item I124"@en-AU ;
    dcat:accessURL <https://www.legislation.gov.au/F2021L00317/asmade/2021-03-24/text/original/epub/OEBPS/document_1/document_1.html#_Toc66194881> ;
    dcat:landingPage "https://www.legislation.gov.au/F2021L00317/asmade/2021-03-24/text/original/epub/OEBPS/document_1/document_1.html#_Toc66194881"^^xsd:anyURI ;
    dcat:theme legcons:Item .

F2021L00317:125 a legcons:Item,
        owl:Class,
        dcat:Resource ;
    rdfs:label "Item - I125 5 45  Information and declarations not received or inaccurate or incomplete"@en-AU ;
    dct:isPartOf F2021L00317:72 ;
    dct:isReferencedBy F2021L00317: ;
    rdfs:comment "5 45  Information and declarations not received or inaccurate or incomplete - Abrievated Graph Key: I125"@en-AU ;
    skos:definition "5 45  Information and declarations not received or inaccurate or incomplete"@en-AU ;
    skos:narrower F2021L00317:72 ;
    skos:prefLabel "Item I125"@en-AU ;
    dcat:accessURL <https://www.legislation.gov.au/F2021L00317/asmade/2021-03-24/text/original/epub/OEBPS/document_1/document_1.html#_Toc66194882> ;
    dcat:landingPage "https://www.legislation.gov.au/F2021L00317/asmade/2021-03-24/text/original/epub/OEBPS/document_1/document_1.html#_Toc66194882"^^xsd:anyURI ;
    dcat:theme legcons:Item .

F2021L00317:126 a legcons:Division,
        owl:Class,
        dcat:Resource ;
    rdfs:label "Division - D126 Division 9 Management practicesexport operations"@en-AU ;
    dct:isPartOf F2021L00317:72 ;
    dct:isReferencedBy F2021L00317: ;
    rdfs:comment "Division 9 Management practicesexport operations - Abrievated Graph Key: D126"@en-AU ;
    skos:definition "Division 9 Management practicesexport operations"@en-AU ;
    skos:narrower F2021L00317:72 ;
    skos:prefLabel "Division D126"@en-AU ;
    dcat:accessURL <https://www.legislation.gov.au/F2021L00317/asmade/2021-03-24/text/original/epub/OEBPS/document_1/document_1.html#_Toc66194883> ;
    dcat:landingPage "https://www.legislation.gov.au/F2021L00317/asmade/2021-03-24/text/original/epub/OEBPS/document_1/document_1.html#_Toc66194883"^^xsd:anyURI ;
    dcat:theme legcons:Division .

F2021L00317:127 a legcons:Item,
        owl:Class,
        dcat:Resource ;
    rdfs:label "Item - I127 5 46  Management practices organisational structure resources and personnel"@en-AU ;
    dct:isPartOf F2021L00317:72 ;
    dct:isReferencedBy F2021L00317: ;
    rdfs:comment "5 46  Management practices organisational structure resources and personnel - Abrievated Graph Key: I127"@en-AU ;
    skos:definition "5 46  Management practices organisational structure resources and personnel"@en-AU ;
    skos:narrower F2021L00317:72 ;
    skos:prefLabel "Item I127"@en-AU ;
    dcat:accessURL <https://www.legislation.gov.au/F2021L00317/asmade/2021-03-24/text/original/epub/OEBPS/document_1/document_1.html#_Toc66194884> ;
    dcat:landingPage "https://www.legislation.gov.au/F2021L00317/asmade/2021-03-24/text/original/epub/OEBPS/document_1/document_1.html#_Toc66194884"^^xsd:anyURI ;
    dcat:theme legcons:Item .

F2021L00317:128 a legcons:Item,
        owl:Class,
        dcat:Resource ;
    rdfs:label "Item - I128 5 47  Verification of compliance with the Act and other matters"@en-AU ;
    dct:isPartOf F2021L00317:72 ;
    dct:isReferencedBy F2021L00317: ;
    rdfs:comment "5 47  Verification of compliance with the Act and other matters - Abrievated Graph Key: I128"@en-AU ;
    skos:definition "5 47  Verification of compliance with the Act and other matters"@en-AU ;
    skos:narrower F2021L00317:72 ;
    skos:prefLabel "Item I128"@en-AU ;
    dcat:accessURL <https://www.legislation.gov.au/F2021L00317/asmade/2021-03-24/text/original/epub/OEBPS/document_1/document_1.html#_Toc66194885> ;
    dcat:landingPage "https://www.legislation.gov.au/F2021L00317/asmade/2021-03-24/text/original/epub/OEBPS/document_1/document_1.html#_Toc66194885"^^xsd:anyURI ;
    dcat:theme legcons:Item .

F2021L00317:129 a legcons:Item,
        owl:Class,
        dcat:Resource ;
    rdfs:label "Item - I129 5 48  Action must be taken to address non compliance"@en-AU ;
    dct:isPartOf F2021L00317:72 ;
    dct:isReferencedBy F2021L00317: ;
    rdfs:comment "5 48  Action must be taken to address non compliance - Abrievated Graph Key: I129"@en-AU ;
    skos:definition "5 48  Action must be taken to address non compliance"@en-AU ;
    skos:narrower F2021L00317:72 ;
    skos:prefLabel "Item I129"@en-AU ;
    dcat:accessURL <https://www.legislation.gov.au/F2021L00317/asmade/2021-03-24/text/original/epub/OEBPS/document_1/document_1.html#_Toc66194886> ;
    dcat:landingPage "https://www.legislation.gov.au/F2021L00317/asmade/2021-03-24/text/original/epub/OEBPS/document_1/document_1.html#_Toc66194886"^^xsd:anyURI ;
    dcat:theme legcons:Item .

F2021L00317:130 a legcons:Item,
        owl:Class,
        dcat:Resource ;
    rdfs:label "Item - I130 5 49  Internal audit and management review"@en-AU ;
    dct:isPartOf F2021L00317:72 ;
    dct:isReferencedBy F2021L00317: ;
    rdfs:comment "5 49  Internal audit and management review - Abrievated Graph Key: I130"@en-AU ;
    skos:definition "5 49  Internal audit and management review"@en-AU ;
    skos:narrower F2021L00317:72 ;
    skos:prefLabel "Item I130"@en-AU ;
    dcat:accessURL <https://www.legislation.gov.au/F2021L00317/asmade/2021-03-24/text/original/epub/OEBPS/document_1/document_1.html#_Toc66194887> ;
    dcat:landingPage "https://www.legislation.gov.au/F2021L00317/asmade/2021-03-24/text/original/epub/OEBPS/document_1/document_1.html#_Toc66194887"^^xsd:anyURI ;
    dcat:theme legcons:Item .

F2021L00317:131 a legcons:Item,
        owl:Class,
        dcat:Resource ;
    rdfs:label "Item - I131 5 50  Authorised officer must be notified if prescribed fish or fish products are not fit for human consumption or integrity cannot be ensured etc"@en-AU ;
    dct:isPartOf F2021L00317:72 ;
    dct:isReferencedBy F2021L00317: ;
    rdfs:comment "5 50  Authorised officer must be notified if prescribed fish or fish products are not fit for human consumption or integrity cannot be ensured etc - Abrievated Graph Key: I131"@en-AU ;
    skos:definition "5 50  Authorised officer must be notified if prescribed fish or fish products are not fit for human consumption or integrity cannot be ensured etc"@en-AU ;
    skos:narrower F2021L00317:72 ;
    skos:prefLabel "Item I131"@en-AU ;
    dcat:accessURL <https://www.legislation.gov.au/F2021L00317/asmade/2021-03-24/text/original/epub/OEBPS/document_1/document_1.html#_Toc66194888> ;
    dcat:landingPage "https://www.legislation.gov.au/F2021L00317/asmade/2021-03-24/text/original/epub/OEBPS/document_1/document_1.html#_Toc66194888"^^xsd:anyURI ;
    dcat:theme legcons:Item .

F2021L00317:132 a legcons:Part,
        owl:Class,
        dcat:Resource ;
    rdfs:label "Part - P132 Part 3 Renewal of approved arrangement"@en-AU ;
    dct:isPartOf F2021L00317:65 ;
    dct:isReferencedBy F2021L00317: ;
    rdfs:comment "Part 3 Renewal of approved arrangement - Abrievated Graph Key: P132"@en-AU ;
    skos:definition "Part 3 Renewal of approved arrangement"@en-AU ;
    skos:narrower F2021L00317:65 ;
    skos:prefLabel "Part P132"@en-AU ;
    dcat:accessURL <https://www.legislation.gov.au/F2021L00317/asmade/2021-03-24/text/original/epub/OEBPS/document_1/document_1.html#_Toc66194889> ;
    dcat:landingPage "https://www.legislation.gov.au/F2021L00317/asmade/2021-03-24/text/original/epub/OEBPS/document_1/document_1.html#_Toc66194889"^^xsd:anyURI ;
    dcat:theme legcons:Part .

F2021L00317:133 a legcons:Item,
        owl:Class,
        dcat:Resource ;
    rdfs:label "Item - I133 5 51  Period within which application to renew approved arrangement must be made"@en-AU ;
    dct:isPartOf F2021L00317:65 ;
    dct:isReferencedBy F2021L00317: ;
    rdfs:comment "5 51  Period within which application to renew approved arrangement must be made - Abrievated Graph Key: I133"@en-AU ;
    skos:definition "5 51  Period within which application to renew approved arrangement must be made"@en-AU ;
    skos:narrower F2021L00317:65 ;
    skos:prefLabel "Item I133"@en-AU ;
    dcat:accessURL <https://www.legislation.gov.au/F2021L00317/asmade/2021-03-24/text/original/epub/OEBPS/document_1/document_1.html#_Toc66194890> ;
    dcat:landingPage "https://www.legislation.gov.au/F2021L00317/asmade/2021-03-24/text/original/epub/OEBPS/document_1/document_1.html#_Toc66194890"^^xsd:anyURI ;
    dcat:theme legcons:Item .

F2021L00317:134 a legcons:Part,
        owl:Class,
        dcat:Resource ;
    rdfs:label "Part - P134 Part 4 Variation of approved arrangement"@en-AU ;
    dct:isPartOf F2021L00317:65 ;
    dct:isReferencedBy F2021L00317: ;
    rdfs:comment "Part 4 Variation of approved arrangement - Abrievated Graph Key: P134"@en-AU ;
    skos:definition "Part 4 Variation of approved arrangement"@en-AU ;
    skos:narrower F2021L00317:65 ;
    skos:prefLabel "Part P134"@en-AU ;
    dcat:accessURL <https://www.legislation.gov.au/F2021L00317/asmade/2021-03-24/text/original/epub/OEBPS/document_1/document_1.html#_Toc66194891> ;
    dcat:landingPage "https://www.legislation.gov.au/F2021L00317/asmade/2021-03-24/text/original/epub/OEBPS/document_1/document_1.html#_Toc66194891"^^xsd:anyURI ;
    dcat:theme legcons:Part .

F2021L00317:136 a legcons:Item,
        owl:Class,
        dcat:Resource ;
    rdfs:label "Item - I136 5 52  Requirements that must be met for variation to be approved or conditions varied"@en-AU ;
    dct:isPartOf F2021L00317:135 ;
    dct:isReferencedBy F2021L00317: ;
    rdfs:comment "5 52  Requirements that must be met for variation to be approved or conditions varied - Abrievated Graph Key: I136"@en-AU ;
    skos:definition "5 52  Requirements that must be met for variation to be approved or conditions varied"@en-AU ;
    skos:narrower F2021L00317:135 ;
    skos:prefLabel "Item I136"@en-AU ;
    dcat:accessURL <https://www.legislation.gov.au/F2021L00317/asmade/2021-03-24/text/original/epub/OEBPS/document_1/document_1.html#_Toc66194893> ;
    dcat:landingPage "https://www.legislation.gov.au/F2021L00317/asmade/2021-03-24/text/original/epub/OEBPS/document_1/document_1.html#_Toc66194893"^^xsd:anyURI ;
    dcat:theme legcons:Item .

F2021L00317:137 a legcons:Item,
        owl:Class,
        dcat:Resource ;
    rdfs:label "Item - I137 5 53  Significant variations"@en-AU ;
    dct:isPartOf F2021L00317:135 ;
    dct:isReferencedBy F2021L00317: ;
    rdfs:comment "5 53  Significant variations - Abrievated Graph Key: I137"@en-AU ;
    skos:definition "5 53  Significant variations"@en-AU ;
    skos:narrower F2021L00317:135 ;
    skos:prefLabel "Item I137"@en-AU ;
    dcat:accessURL <https://www.legislation.gov.au/F2021L00317/asmade/2021-03-24/text/original/epub/OEBPS/document_1/document_1.html#_Toc66194894> ;
    dcat:landingPage "https://www.legislation.gov.au/F2021L00317/asmade/2021-03-24/text/original/epub/OEBPS/document_1/document_1.html#_Toc66194894"^^xsd:anyURI ;
    dcat:theme legcons:Item .

F2021L00317:139 a legcons:Item,
        owl:Class,
        dcat:Resource ;
    rdfs:label "Item - I139 5 54  Other reasons for requiring holder to vary approved arrangement"@en-AU ;
    dct:isPartOf F2021L00317:138 ;
    dct:isReferencedBy F2021L00317: ;
    rdfs:comment "5 54  Other reasons for requiring holder to vary approved arrangement - Abrievated Graph Key: I139"@en-AU ;
    skos:definition "5 54  Other reasons for requiring holder to vary approved arrangement"@en-AU ;
    skos:narrower F2021L00317:138 ;
    skos:prefLabel "Item I139"@en-AU ;
    dcat:accessURL <https://www.legislation.gov.au/F2021L00317/asmade/2021-03-24/text/original/epub/OEBPS/document_1/document_1.html#_Toc66194896> ;
    dcat:landingPage "https://www.legislation.gov.au/F2021L00317/asmade/2021-03-24/text/original/epub/OEBPS/document_1/document_1.html#_Toc66194896"^^xsd:anyURI ;
    dcat:theme legcons:Item .

F2021L00317:14 a legcons:Item,
        owl:Class,
        dcat:Resource ;
    rdfs:label "Item - I14 2 1  Fish and fish products that are prescribed goods"@en-AU ;
    dct:isPartOf F2021L00317:13 ;
    dct:isReferencedBy F2021L00317: ;
    rdfs:comment "2 1  Fish and fish products that are prescribed goods - Abrievated Graph Key: I14"@en-AU ;
    skos:definition "2 1  Fish and fish products that are prescribed goods"@en-AU ;
    skos:narrower F2021L00317:13 ;
    skos:prefLabel "Item I14"@en-AU ;
    dcat:accessURL <https://www.legislation.gov.au/F2021L00317/asmade/2021-03-24/text/original/epub/OEBPS/document_1/document_1.html#_Toc66194771> ;
    dcat:landingPage "https://www.legislation.gov.au/F2021L00317/asmade/2021-03-24/text/original/epub/OEBPS/document_1/document_1.html#_Toc66194771"^^xsd:anyURI ;
    dcat:theme legcons:Item .

F2021L00317:140 a legcons:Part,
        owl:Class,
        dcat:Resource ;
    rdfs:label "Part - P140 Part 5 Matters relating to applications"@en-AU ;
    dct:isPartOf F2021L00317:65 ;
    dct:isReferencedBy F2021L00317: ;
    rdfs:comment "Part 5 Matters relating to applications - Abrievated Graph Key: P140"@en-AU ;
    skos:definition "Part 5 Matters relating to applications"@en-AU ;
    skos:narrower F2021L00317:65 ;
    skos:prefLabel "Part P140"@en-AU ;
    dcat:accessURL <https://www.legislation.gov.au/F2021L00317/asmade/2021-03-24/text/original/epub/OEBPS/document_1/document_1.html#_Toc66194897> ;
    dcat:landingPage "https://www.legislation.gov.au/F2021L00317/asmade/2021-03-24/text/original/epub/OEBPS/document_1/document_1.html#_Toc66194897"^^xsd:anyURI ;
    dcat:theme legcons:Part .

F2021L00317:141 a legcons:Item,
        owl:Class,
        dcat:Resource ;
    rdfs:label "Item - I141 5 55  Application of this Part"@en-AU ;
    dct:isPartOf F2021L00317:65 ;
    dct:isReferencedBy F2021L00317: ;
    rdfs:comment "5 55  Application of this Part - Abrievated Graph Key: I141"@en-AU ;
    skos:definition "5 55  Application of this Part"@en-AU ;
    skos:narrower F2021L00317:65 ;
    skos:prefLabel "Item I141"@en-AU ;
    dcat:accessURL <https://www.legislation.gov.au/F2021L00317/asmade/2021-03-24/text/original/epub/OEBPS/document_1/document_1.html#_Toc66194898> ;
    dcat:landingPage "https://www.legislation.gov.au/F2021L00317/asmade/2021-03-24/text/original/epub/OEBPS/document_1/document_1.html#_Toc66194898"^^xsd:anyURI ;
    dcat:theme legcons:Item .

F2021L00317:142 a legcons:Item,
        owl:Class,
        dcat:Resource ;
    rdfs:label "Item - I142 5 56  Initial consideration period"@en-AU ;
    dct:isPartOf F2021L00317:65 ;
    dct:isReferencedBy F2021L00317: ;
    rdfs:comment "5 56  Initial consideration period - Abrievated Graph Key: I142"@en-AU ;
    skos:definition "5 56  Initial consideration period"@en-AU ;
    skos:narrower F2021L00317:65 ;
    skos:prefLabel "Item I142"@en-AU ;
    dcat:accessURL <https://www.legislation.gov.au/F2021L00317/asmade/2021-03-24/text/original/epub/OEBPS/document_1/document_1.html#_Toc66194899> ;
    dcat:landingPage "https://www.legislation.gov.au/F2021L00317/asmade/2021-03-24/text/original/epub/OEBPS/document_1/document_1.html#_Toc66194899"^^xsd:anyURI ;
    dcat:theme legcons:Item .

F2021L00317:143 a legcons:Item,
        owl:Class,
        dcat:Resource ;
    rdfs:label "Item - I143 5 57  Period within which request relating to application must be complied with"@en-AU ;
    dct:isPartOf F2021L00317:65 ;
    dct:isReferencedBy F2021L00317: ;
    rdfs:comment "5 57  Period within which request relating to application must be complied with - Abrievated Graph Key: I143"@en-AU ;
    skos:definition "5 57  Period within which request relating to application must be complied with"@en-AU ;
    skos:narrower F2021L00317:65 ;
    skos:prefLabel "Item I143"@en-AU ;
    dcat:accessURL <https://www.legislation.gov.au/F2021L00317/asmade/2021-03-24/text/original/epub/OEBPS/document_1/document_1.html#_Toc66194900> ;
    dcat:landingPage "https://www.legislation.gov.au/F2021L00317/asmade/2021-03-24/text/original/epub/OEBPS/document_1/document_1.html#_Toc66194900"^^xsd:anyURI ;
    dcat:theme legcons:Item .

F2021L00317:146 a legcons:Item,
        owl:Class,
        dcat:Resource ;
    rdfs:label "Item - I146 7 1  Conditions of export permit"@en-AU ;
    dct:isPartOf F2021L00317:145 ;
    dct:isReferencedBy F2021L00317: ;
    rdfs:comment "7 1  Conditions of export permit - Abrievated Graph Key: I146"@en-AU ;
    skos:definition "7 1  Conditions of export permit"@en-AU ;
    skos:narrower F2021L00317:145 ;
    skos:prefLabel "Item I146"@en-AU ;
    dcat:accessURL <https://www.legislation.gov.au/F2021L00317/asmade/2021-03-24/text/original/epub/OEBPS/document_1/document_1.html#_Toc66194903> ;
    dcat:landingPage "https://www.legislation.gov.au/F2021L00317/asmade/2021-03-24/text/original/epub/OEBPS/document_1/document_1.html#_Toc66194903"^^xsd:anyURI ;
    dcat:theme legcons:Item .

F2021L00317:147 a legcons:Item,
        owl:Class,
        dcat:Resource ;
    rdfs:label "Item - I147 7 2  Period of effect of export permit"@en-AU ;
    dct:isPartOf F2021L00317:145 ;
    dct:isReferencedBy F2021L00317: ;
    rdfs:comment "7 2  Period of effect of export permit - Abrievated Graph Key: I147"@en-AU ;
    skos:definition "7 2  Period of effect of export permit"@en-AU ;
    skos:narrower F2021L00317:145 ;
    skos:prefLabel "Item I147"@en-AU ;
    dcat:accessURL <https://www.legislation.gov.au/F2021L00317/asmade/2021-03-24/text/original/epub/OEBPS/document_1/document_1.html#_Toc66194904> ;
    dcat:landingPage "https://www.legislation.gov.au/F2021L00317/asmade/2021-03-24/text/original/epub/OEBPS/document_1/document_1.html#_Toc66194904"^^xsd:anyURI ;
    dcat:theme legcons:Item .

F2021L00317:149 a legcons:Item,
        owl:Class,
        dcat:Resource ;
    rdfs:label "Item - I149 7 3  Period of effect of varied export permit"@en-AU ;
    dct:isPartOf F2021L00317:148 ;
    dct:isReferencedBy F2021L00317: ;
    rdfs:comment "7 3  Period of effect of varied export permit - Abrievated Graph Key: I149"@en-AU ;
    skos:definition "7 3  Period of effect of varied export permit"@en-AU ;
    skos:narrower F2021L00317:148 ;
    skos:prefLabel "Item I149"@en-AU ;
    dcat:accessURL <https://www.legislation.gov.au/F2021L00317/asmade/2021-03-24/text/original/epub/OEBPS/document_1/document_1.html#_Toc66194906> ;
    dcat:landingPage "https://www.legislation.gov.au/F2021L00317/asmade/2021-03-24/text/original/epub/OEBPS/document_1/document_1.html#_Toc66194906"^^xsd:anyURI ;
    dcat:theme legcons:Item .

F2021L00317:15 a legcons:Item,
        owl:Class,
        dcat:Resource ;
    rdfs:label "Item - I15 2 2  Fish and fish products that are taken not to be prescribed goods"@en-AU ;
    dct:isPartOf F2021L00317:13 ;
    dct:isReferencedBy F2021L00317: ;
    rdfs:comment "2 2  Fish and fish products that are taken not to be prescribed goods - Abrievated Graph Key: I15"@en-AU ;
    skos:definition "2 2  Fish and fish products that are taken not to be prescribed goods"@en-AU ;
    skos:narrower F2021L00317:13 ;
    skos:prefLabel "Item I15"@en-AU ;
    dcat:accessURL <https://www.legislation.gov.au/F2021L00317/asmade/2021-03-24/text/original/epub/OEBPS/document_1/document_1.html#_Toc66194772> ;
    dcat:landingPage "https://www.legislation.gov.au/F2021L00317/asmade/2021-03-24/text/original/epub/OEBPS/document_1/document_1.html#_Toc66194772"^^xsd:anyURI ;
    dcat:theme legcons:Item .

F2021L00317:150 a legcons:Item,
        owl:Class,
        dcat:Resource ;
    rdfs:label "Item - I150 7 4  Circumstances in which export permit may be suspended"@en-AU ;
    dct:isPartOf F2021L00317:148 ;
    dct:isReferencedBy F2021L00317: ;
    rdfs:comment "7 4  Circumstances in which export permit may be suspended - Abrievated Graph Key: I150"@en-AU ;
    skos:definition "7 4  Circumstances in which export permit may be suspended"@en-AU ;
    skos:narrower F2021L00317:148 ;
    skos:prefLabel "Item I150"@en-AU ;
    dcat:accessURL <https://www.legislation.gov.au/F2021L00317/asmade/2021-03-24/text/original/epub/OEBPS/document_1/document_1.html#_Toc66194907> ;
    dcat:landingPage "https://www.legislation.gov.au/F2021L00317/asmade/2021-03-24/text/original/epub/OEBPS/document_1/document_1.html#_Toc66194907"^^xsd:anyURI ;
    dcat:theme legcons:Item .

F2021L00317:151 a legcons:Item,
        owl:Class,
        dcat:Resource ;
    rdfs:label "Item - I151 7 5  Other circumstances in which export permit may be revoked"@en-AU ;
    dct:isPartOf F2021L00317:148 ;
    dct:isReferencedBy F2021L00317: ;
    rdfs:comment "7 5  Other circumstances in which export permit may be revoked - Abrievated Graph Key: I151"@en-AU ;
    skos:definition "7 5  Other circumstances in which export permit may be revoked"@en-AU ;
    skos:narrower F2021L00317:148 ;
    skos:prefLabel "Item I151"@en-AU ;
    dcat:accessURL <https://www.legislation.gov.au/F2021L00317/asmade/2021-03-24/text/original/epub/OEBPS/document_1/document_1.html#_Toc66194908> ;
    dcat:landingPage "https://www.legislation.gov.au/F2021L00317/asmade/2021-03-24/text/original/epub/OEBPS/document_1/document_1.html#_Toc66194908"^^xsd:anyURI ;
    dcat:theme legcons:Item .

F2021L00317:153 a legcons:Item,
        owl:Class,
        dcat:Resource ;
    rdfs:label "Item - I153 7 6  Changes that require additional or corrected information to be given to the Secretary"@en-AU ;
    dct:isPartOf F2021L00317:152 ;
    dct:isReferencedBy F2021L00317: ;
    rdfs:comment "7 6  Changes that require additional or corrected information to be given to the Secretary - Abrievated Graph Key: I153"@en-AU ;
    skos:definition "7 6  Changes that require additional or corrected information to be given to the Secretary"@en-AU ;
    skos:narrower F2021L00317:152 ;
    skos:prefLabel "Item I153"@en-AU ;
    dcat:accessURL <https://www.legislation.gov.au/F2021L00317/asmade/2021-03-24/text/original/epub/OEBPS/document_1/document_1.html#_Toc66194910> ;
    dcat:landingPage "https://www.legislation.gov.au/F2021L00317/asmade/2021-03-24/text/original/epub/OEBPS/document_1/document_1.html#_Toc66194910"^^xsd:anyURI ;
    dcat:theme legcons:Item .

F2021L00317:154 a legcons:Item,
        owl:Class,
        dcat:Resource ;
    rdfs:label "Item - I154 7 7  Return of export permit"@en-AU ;
    dct:isPartOf F2021L00317:152 ;
    dct:isReferencedBy F2021L00317: ;
    rdfs:comment "7 7  Return of export permit - Abrievated Graph Key: I154"@en-AU ;
    skos:definition "7 7  Return of export permit"@en-AU ;
    skos:narrower F2021L00317:152 ;
    skos:prefLabel "Item I154"@en-AU ;
    dcat:accessURL <https://www.legislation.gov.au/F2021L00317/asmade/2021-03-24/text/original/epub/OEBPS/document_1/document_1.html#_Toc66194911> ;
    dcat:landingPage "https://www.legislation.gov.au/F2021L00317/asmade/2021-03-24/text/original/epub/OEBPS/document_1/document_1.html#_Toc66194911"^^xsd:anyURI ;
    dcat:theme legcons:Item .

F2021L00317:155 a legcons:Item,
        owl:Class,
        dcat:Resource ;
    rdfs:label "Item - I155 7 8  Notification that prescribed fish or fish products are not to be exported"@en-AU ;
    dct:isPartOf F2021L00317:152 ;
    dct:isReferencedBy F2021L00317: ;
    rdfs:comment "7 8  Notification that prescribed fish or fish products are not to be exported - Abrievated Graph Key: I155"@en-AU ;
    skos:definition "7 8  Notification that prescribed fish or fish products are not to be exported"@en-AU ;
    skos:narrower F2021L00317:152 ;
    skos:prefLabel "Item I155"@en-AU ;
    dcat:accessURL <https://www.legislation.gov.au/F2021L00317/asmade/2021-03-24/text/original/epub/OEBPS/document_1/document_1.html#_Toc66194912> ;
    dcat:landingPage "https://www.legislation.gov.au/F2021L00317/asmade/2021-03-24/text/original/epub/OEBPS/document_1/document_1.html#_Toc66194912"^^xsd:anyURI ;
    dcat:theme legcons:Item .

F2021L00317:157 a legcons:Item,
        owl:Class,
        dcat:Resource ;
    rdfs:label "Item - I157 7 9  Application of this Part"@en-AU ;
    dct:isPartOf F2021L00317:156 ;
    dct:isReferencedBy F2021L00317: ;
    rdfs:comment "7 9  Application of this Part - Abrievated Graph Key: I157"@en-AU ;
    skos:definition "7 9  Application of this Part"@en-AU ;
    skos:narrower F2021L00317:156 ;
    skos:prefLabel "Item I157"@en-AU ;
    dcat:accessURL <https://www.legislation.gov.au/F2021L00317/asmade/2021-03-24/text/original/epub/OEBPS/document_1/document_1.html#_Toc66194914> ;
    dcat:landingPage "https://www.legislation.gov.au/F2021L00317/asmade/2021-03-24/text/original/epub/OEBPS/document_1/document_1.html#_Toc66194914"^^xsd:anyURI ;
    dcat:theme legcons:Item .

F2021L00317:158 a legcons:Item,
        owl:Class,
        dcat:Resource ;
    rdfs:label "Item - I158 7 10  Documents to accompany application"@en-AU ;
    dct:isPartOf F2021L00317:156 ;
    dct:isReferencedBy F2021L00317: ;
    rdfs:comment "7 10  Documents to accompany application - Abrievated Graph Key: I158"@en-AU ;
    skos:definition "7 10  Documents to accompany application"@en-AU ;
    skos:narrower F2021L00317:156 ;
    skos:prefLabel "Item I158"@en-AU ;
    dcat:accessURL <https://www.legislation.gov.au/F2021L00317/asmade/2021-03-24/text/original/epub/OEBPS/document_1/document_1.html#_Toc66194915> ;
    dcat:landingPage "https://www.legislation.gov.au/F2021L00317/asmade/2021-03-24/text/original/epub/OEBPS/document_1/document_1.html#_Toc66194915"^^xsd:anyURI ;
    dcat:theme legcons:Item .

F2021L00317:16 a legcons:Division,
        owl:Class,
        dcat:Resource ;
    rdfs:label "Division - D16 Division 2 Prohibited export and prescribed export conditions"@en-AU ;
    dct:isPartOf F2021L00317:12 ;
    dct:isReferencedBy F2021L00317: ;
    rdfs:comment "Division 2 Prohibited export and prescribed export conditions - Abrievated Graph Key: D16"@en-AU ;
    skos:definition "Division 2 Prohibited export and prescribed export conditions"@en-AU ;
    skos:narrower F2021L00317:12 ;
    skos:prefLabel "Division D16"@en-AU ;
    dcat:accessURL <https://www.legislation.gov.au/F2021L00317/asmade/2021-03-24/text/original/epub/OEBPS/document_1/document_1.html#_Toc66194773> ;
    dcat:landingPage "https://www.legislation.gov.au/F2021L00317/asmade/2021-03-24/text/original/epub/OEBPS/document_1/document_1.html#_Toc66194773"^^xsd:anyURI ;
    dcat:theme legcons:Division .

F2021L00317:161 a legcons:Item,
        owl:Class,
        dcat:Resource ;
    rdfs:label "Item - I161 8 1  Purpose of this Part"@en-AU ;
    dct:isPartOf F2021L00317:160 ;
    dct:isReferencedBy F2021L00317: ;
    rdfs:comment "8 1  Purpose of this Part - Abrievated Graph Key: I161"@en-AU ;
    skos:definition "8 1  Purpose of this Part"@en-AU ;
    skos:narrower F2021L00317:160 ;
    skos:prefLabel "Item I161"@en-AU ;
    dcat:accessURL <https://www.legislation.gov.au/F2021L00317/asmade/2021-03-24/text/original/epub/OEBPS/document_1/document_1.html#_Toc66194918> ;
    dcat:landingPage "https://www.legislation.gov.au/F2021L00317/asmade/2021-03-24/text/original/epub/OEBPS/document_1/document_1.html#_Toc66194918"^^xsd:anyURI ;
    dcat:theme legcons:Item .

F2021L00317:162 a legcons:Item,
        owl:Class,
        dcat:Resource ;
    rdfs:label "Item - I162 8 2  General requirements for trade descriptions"@en-AU ;
    dct:isPartOf F2021L00317:160 ;
    dct:isReferencedBy F2021L00317: ;
    rdfs:comment "8 2  General requirements for trade descriptions - Abrievated Graph Key: I162"@en-AU ;
    skos:definition "8 2  General requirements for trade descriptions"@en-AU ;
    skos:narrower F2021L00317:160 ;
    skos:prefLabel "Item I162"@en-AU ;
    dcat:accessURL <https://www.legislation.gov.au/F2021L00317/asmade/2021-03-24/text/original/epub/OEBPS/document_1/document_1.html#_Toc66194919> ;
    dcat:landingPage "https://www.legislation.gov.au/F2021L00317/asmade/2021-03-24/text/original/epub/OEBPS/document_1/document_1.html#_Toc66194919"^^xsd:anyURI ;
    dcat:theme legcons:Item .

F2021L00317:163 a legcons:Item,
        owl:Class,
        dcat:Resource ;
    rdfs:label "Item - I163 8 3  Trade descriptions in language other than English"@en-AU ;
    dct:isPartOf F2021L00317:160 ;
    dct:isReferencedBy F2021L00317: ;
    rdfs:comment "8 3  Trade descriptions in language other than English - Abrievated Graph Key: I163"@en-AU ;
    skos:definition "8 3  Trade descriptions in language other than English"@en-AU ;
    skos:narrower F2021L00317:160 ;
    skos:prefLabel "Item I163"@en-AU ;
    dcat:accessURL <https://www.legislation.gov.au/F2021L00317/asmade/2021-03-24/text/original/epub/OEBPS/document_1/document_1.html#_Toc66194920> ;
    dcat:landingPage "https://www.legislation.gov.au/F2021L00317/asmade/2021-03-24/text/original/epub/OEBPS/document_1/document_1.html#_Toc66194920"^^xsd:anyURI ;
    dcat:theme legcons:Item .

F2021L00317:166 a legcons:Item,
        owl:Class,
        dcat:Resource ;
    rdfs:label "Item - I166 8 4  Purpose of this Division"@en-AU ;
    dct:isPartOf F2021L00317:165 ;
    dct:isReferencedBy F2021L00317: ;
    rdfs:comment "8 4  Purpose of this Division - Abrievated Graph Key: I166"@en-AU ;
    skos:definition "8 4  Purpose of this Division"@en-AU ;
    skos:narrower F2021L00317:165 ;
    skos:prefLabel "Item I166"@en-AU ;
    dcat:accessURL <https://www.legislation.gov.au/F2021L00317/asmade/2021-03-24/text/original/epub/OEBPS/document_1/document_1.html#_Toc66194923> ;
    dcat:landingPage "https://www.legislation.gov.au/F2021L00317/asmade/2021-03-24/text/original/epub/OEBPS/document_1/document_1.html#_Toc66194923"^^xsd:anyURI ;
    dcat:theme legcons:Item .

F2021L00317:167 a legcons:Item,
        owl:Class,
        dcat:Resource ;
    rdfs:label "Item - I167 8 5  Tolerances for dimensions of official marks"@en-AU ;
    dct:isPartOf F2021L00317:165 ;
    dct:isReferencedBy F2021L00317: ;
    rdfs:comment "8 5  Tolerances for dimensions of official marks - Abrievated Graph Key: I167"@en-AU ;
    skos:definition "8 5  Tolerances for dimensions of official marks"@en-AU ;
    skos:narrower F2021L00317:165 ;
    skos:prefLabel "Item I167"@en-AU ;
    dcat:accessURL <https://www.legislation.gov.au/F2021L00317/asmade/2021-03-24/text/original/epub/OEBPS/document_1/document_1.html#_Toc66194924> ;
    dcat:landingPage "https://www.legislation.gov.au/F2021L00317/asmade/2021-03-24/text/original/epub/OEBPS/document_1/document_1.html#_Toc66194924"^^xsd:anyURI ;
    dcat:theme legcons:Item .

F2021L00317:168 a legcons:Item,
        owl:Class,
        dcat:Resource ;
    rdfs:label "Item - I168 8 6  Official markforeign country identification"@en-AU ;
    dct:isPartOf F2021L00317:165 ;
    dct:isReferencedBy F2021L00317: ;
    rdfs:comment "8 6  Official markforeign country identification - Abrievated Graph Key: I168"@en-AU ;
    skos:definition "8 6  Official markforeign country identification"@en-AU ;
    skos:narrower F2021L00317:165 ;
    skos:prefLabel "Item I168"@en-AU ;
    dcat:accessURL <https://www.legislation.gov.au/F2021L00317/asmade/2021-03-24/text/original/epub/OEBPS/document_1/document_1.html#_Toc66194925> ;
    dcat:landingPage "https://www.legislation.gov.au/F2021L00317/asmade/2021-03-24/text/original/epub/OEBPS/document_1/document_1.html#_Toc66194925"^^xsd:anyURI ;
    dcat:theme legcons:Item .

F2021L00317:169 a legcons:Item,
        owl:Class,
        dcat:Resource ;
    rdfs:label "Item - I169 8 7  Official marktamper indicative metal strap seal"@en-AU ;
    dct:isPartOf F2021L00317:165 ;
    dct:isReferencedBy F2021L00317: ;
    rdfs:comment "8 7  Official marktamper indicative metal strap seal - Abrievated Graph Key: I169"@en-AU ;
    skos:definition "8 7  Official marktamper indicative metal strap seal"@en-AU ;
    skos:narrower F2021L00317:165 ;
    skos:prefLabel "Item I169"@en-AU ;
    dcat:accessURL <https://www.legislation.gov.au/F2021L00317/asmade/2021-03-24/text/original/epub/OEBPS/document_1/document_1.html#_Toc66194926> ;
    dcat:landingPage "https://www.legislation.gov.au/F2021L00317/asmade/2021-03-24/text/original/epub/OEBPS/document_1/document_1.html#_Toc66194926"^^xsd:anyURI ;
    dcat:theme legcons:Item .

F2021L00317:17 a legcons:Item,
        owl:Class,
        dcat:Resource ;
    rdfs:label "Item - I17 2 3  Purpose and application of this Division"@en-AU ;
    dct:isPartOf F2021L00317:12 ;
    dct:isReferencedBy F2021L00317: ;
    rdfs:comment "2 3  Purpose and application of this Division - Abrievated Graph Key: I17"@en-AU ;
    skos:definition "2 3  Purpose and application of this Division"@en-AU ;
    skos:narrower F2021L00317:12 ;
    skos:prefLabel "Item I17"@en-AU ;
    dcat:accessURL <https://www.legislation.gov.au/F2021L00317/asmade/2021-03-24/text/original/epub/OEBPS/document_1/document_1.html#_Toc66194774> ;
    dcat:landingPage "https://www.legislation.gov.au/F2021L00317/asmade/2021-03-24/text/original/epub/OEBPS/document_1/document_1.html#_Toc66194774"^^xsd:anyURI ;
    dcat:theme legcons:Item .

F2021L00317:170 a legcons:Item,
        owl:Class,
        dcat:Resource ;
    rdfs:label "Item - I170 8 8  Official markbolt seal"@en-AU ;
    dct:isPartOf F2021L00317:165 ;
    dct:isReferencedBy F2021L00317: ;
    rdfs:comment "8 8  Official markbolt seal - Abrievated Graph Key: I170"@en-AU ;
    skos:definition "8 8  Official markbolt seal"@en-AU ;
    skos:narrower F2021L00317:165 ;
    skos:prefLabel "Item I170"@en-AU ;
    dcat:accessURL <https://www.legislation.gov.au/F2021L00317/asmade/2021-03-24/text/original/epub/OEBPS/document_1/document_1.html#_Toc66194927> ;
    dcat:landingPage "https://www.legislation.gov.au/F2021L00317/asmade/2021-03-24/text/original/epub/OEBPS/document_1/document_1.html#_Toc66194927"^^xsd:anyURI ;
    dcat:theme legcons:Item .

F2021L00317:171 a legcons:Item,
        owl:Class,
        dcat:Resource ;
    rdfs:label "Item - I171 8 9  Official markEuropean Union"@en-AU ;
    dct:isPartOf F2021L00317:165 ;
    dct:isReferencedBy F2021L00317: ;
    rdfs:comment "8 9  Official markEuropean Union - Abrievated Graph Key: I171"@en-AU ;
    skos:definition "8 9  Official markEuropean Union"@en-AU ;
    skos:narrower F2021L00317:165 ;
    skos:prefLabel "Item I171"@en-AU ;
    dcat:accessURL <https://www.legislation.gov.au/F2021L00317/asmade/2021-03-24/text/original/epub/OEBPS/document_1/document_1.html#_Toc66194928> ;
    dcat:landingPage "https://www.legislation.gov.au/F2021L00317/asmade/2021-03-24/text/original/epub/OEBPS/document_1/document_1.html#_Toc66194928"^^xsd:anyURI ;
    dcat:theme legcons:Item .

F2021L00317:172 a legcons:Item,
        owl:Class,
        dcat:Resource ;
    rdfs:label "Item - I172 8 10  Official markcarton seal"@en-AU ;
    dct:isPartOf F2021L00317:165 ;
    dct:isReferencedBy F2021L00317: ;
    rdfs:comment "8 10  Official markcarton seal - Abrievated Graph Key: I172"@en-AU ;
    skos:definition "8 10  Official markcarton seal"@en-AU ;
    skos:narrower F2021L00317:165 ;
    skos:prefLabel "Item I172"@en-AU ;
    dcat:accessURL <https://www.legislation.gov.au/F2021L00317/asmade/2021-03-24/text/original/epub/OEBPS/document_1/document_1.html#_Toc66194929> ;
    dcat:landingPage "https://www.legislation.gov.au/F2021L00317/asmade/2021-03-24/text/original/epub/OEBPS/document_1/document_1.html#_Toc66194929"^^xsd:anyURI ;
    dcat:theme legcons:Item .

F2021L00317:173 a legcons:Item,
        owl:Class,
        dcat:Resource ;
    rdfs:label "Item - I173 8 11  Official markgoods opened for assessment and resealed"@en-AU ;
    dct:isPartOf F2021L00317:165 ;
    dct:isReferencedBy F2021L00317: ;
    rdfs:comment "8 11  Official markgoods opened for assessment and resealed - Abrievated Graph Key: I173"@en-AU ;
    skos:definition "8 11  Official markgoods opened for assessment and resealed"@en-AU ;
    skos:narrower F2021L00317:165 ;
    skos:prefLabel "Item I173"@en-AU ;
    dcat:accessURL <https://www.legislation.gov.au/F2021L00317/asmade/2021-03-24/text/original/epub/OEBPS/document_1/document_1.html#_Toc66194930> ;
    dcat:landingPage "https://www.legislation.gov.au/F2021L00317/asmade/2021-03-24/text/original/epub/OEBPS/document_1/document_1.html#_Toc66194930"^^xsd:anyURI ;
    dcat:theme legcons:Item .

F2021L00317:174 a legcons:Item,
        owl:Class,
        dcat:Resource ;
    rdfs:label "Item - I174 8 12  Official markAustralian Government"@en-AU ;
    dct:isPartOf F2021L00317:165 ;
    dct:isReferencedBy F2021L00317: ;
    rdfs:comment "8 12  Official markAustralian Government - Abrievated Graph Key: I174"@en-AU ;
    skos:definition "8 12  Official markAustralian Government"@en-AU ;
    skos:narrower F2021L00317:165 ;
    skos:prefLabel "Item I174"@en-AU ;
    dcat:accessURL <https://www.legislation.gov.au/F2021L00317/asmade/2021-03-24/text/original/epub/OEBPS/document_1/document_1.html#_Toc66194931> ;
    dcat:landingPage "https://www.legislation.gov.au/F2021L00317/asmade/2021-03-24/text/original/epub/OEBPS/document_1/document_1.html#_Toc66194931"^^xsd:anyURI ;
    dcat:theme legcons:Item .

F2021L00317:176 a legcons:Item,
        owl:Class,
        dcat:Resource ;
    rdfs:label "Item - I176 8 13  Purpose and application of this Division"@en-AU ;
    dct:isPartOf F2021L00317:175 ;
    dct:isReferencedBy F2021L00317: ;
    rdfs:comment "8 13  Purpose and application of this Division - Abrievated Graph Key: I176"@en-AU ;
    skos:definition "8 13  Purpose and application of this Division"@en-AU ;
    skos:narrower F2021L00317:175 ;
    skos:prefLabel "Item I176"@en-AU ;
    dcat:accessURL <https://www.legislation.gov.au/F2021L00317/asmade/2021-03-24/text/original/epub/OEBPS/document_1/document_1.html#_Toc66194933> ;
    dcat:landingPage "https://www.legislation.gov.au/F2021L00317/asmade/2021-03-24/text/original/epub/OEBPS/document_1/document_1.html#_Toc66194933"^^xsd:anyURI ;
    dcat:theme legcons:Item .

F2021L00317:177 a legcons:Item,
        owl:Class,
        dcat:Resource ;
    rdfs:label "Item - I177 8 14  Interpretation"@en-AU ;
    dct:isPartOf F2021L00317:175 ;
    dct:isReferencedBy F2021L00317: ;
    rdfs:comment "8 14  Interpretation - Abrievated Graph Key: I177"@en-AU ;
    skos:definition "8 14  Interpretation"@en-AU ;
    skos:narrower F2021L00317:175 ;
    skos:prefLabel "Item I177"@en-AU ;
    dcat:accessURL <https://www.legislation.gov.au/F2021L00317/asmade/2021-03-24/text/original/epub/OEBPS/document_1/document_1.html#_Toc66194934> ;
    dcat:landingPage "https://www.legislation.gov.au/F2021L00317/asmade/2021-03-24/text/original/epub/OEBPS/document_1/document_1.html#_Toc66194934"^^xsd:anyURI ;
    dcat:theme legcons:Item .

F2021L00317:178 a legcons:Item,
        owl:Class,
        dcat:Resource ;
    rdfs:label "Item - I178 8 15  Persons who may manufacture or supply official marks for fish or fish products"@en-AU ;
    dct:isPartOf F2021L00317:175 ;
    dct:isReferencedBy F2021L00317: ;
    rdfs:comment "8 15  Persons who may manufacture or supply official marks for fish or fish products - Abrievated Graph Key: I178"@en-AU ;
    skos:definition "8 15  Persons who may manufacture or supply official marks for fish or fish products"@en-AU ;
    skos:narrower F2021L00317:175 ;
    skos:prefLabel "Item I178"@en-AU ;
    dcat:accessURL <https://www.legislation.gov.au/F2021L00317/asmade/2021-03-24/text/original/epub/OEBPS/document_1/document_1.html#_Toc66194935> ;
    dcat:landingPage "https://www.legislation.gov.au/F2021L00317/asmade/2021-03-24/text/original/epub/OEBPS/document_1/document_1.html#_Toc66194935"^^xsd:anyURI ;
    dcat:theme legcons:Item .

F2021L00317:179 a legcons:Item,
        owl:Class,
        dcat:Resource ;
    rdfs:label "Item - I179 8 16  Persons who may possess official marks that have not been applied to fish or fish products"@en-AU ;
    dct:isPartOf F2021L00317:175 ;
    dct:isReferencedBy F2021L00317: ;
    rdfs:comment "8 16  Persons who may possess official marks that have not been applied to fish or fish products - Abrievated Graph Key: I179"@en-AU ;
    skos:definition "8 16  Persons who may possess official marks that have not been applied to fish or fish products"@en-AU ;
    skos:narrower F2021L00317:175 ;
    skos:prefLabel "Item I179"@en-AU ;
    dcat:accessURL <https://www.legislation.gov.au/F2021L00317/asmade/2021-03-24/text/original/epub/OEBPS/document_1/document_1.html#_Toc66194936> ;
    dcat:landingPage "https://www.legislation.gov.au/F2021L00317/asmade/2021-03-24/text/original/epub/OEBPS/document_1/document_1.html#_Toc66194936"^^xsd:anyURI ;
    dcat:theme legcons:Item .

F2021L00317:18 a legcons:Item,
        owl:Class,
        dcat:Resource ;
    rdfs:label "Item - I18 2 4  Export of prescribed fish or fish products is prohibited unless prescribed conditions are complied with"@en-AU ;
    dct:isPartOf F2021L00317:12 ;
    dct:isReferencedBy F2021L00317: ;
    rdfs:comment "2 4  Export of prescribed fish or fish products is prohibited unless prescribed conditions are complied with - Abrievated Graph Key: I18"@en-AU ;
    skos:definition "2 4  Export of prescribed fish or fish products is prohibited unless prescribed conditions are complied with"@en-AU ;
    skos:narrower F2021L00317:12 ;
    skos:prefLabel "Item I18"@en-AU ;
    dcat:accessURL <https://www.legislation.gov.au/F2021L00317/asmade/2021-03-24/text/original/epub/OEBPS/document_1/document_1.html#_Toc66194775> ;
    dcat:landingPage "https://www.legislation.gov.au/F2021L00317/asmade/2021-03-24/text/original/epub/OEBPS/document_1/document_1.html#_Toc66194775"^^xsd:anyURI ;
    dcat:theme legcons:Item .

F2021L00317:180 a legcons:Item,
        owl:Class,
        dcat:Resource ;
    rdfs:label "Item - I180 8 17  Persons who may apply official marks to fish or fish products etc"@en-AU ;
    dct:isPartOf F2021L00317:175 ;
    dct:isReferencedBy F2021L00317: ;
    rdfs:comment "8 17  Persons who may apply official marks to fish or fish products etc - Abrievated Graph Key: I180"@en-AU ;
    skos:definition "8 17  Persons who may apply official marks to fish or fish products etc"@en-AU ;
    skos:narrower F2021L00317:175 ;
    skos:prefLabel "Item I180"@en-AU ;
    dcat:accessURL <https://www.legislation.gov.au/F2021L00317/asmade/2021-03-24/text/original/epub/OEBPS/document_1/document_1.html#_Toc66194937> ;
    dcat:landingPage "https://www.legislation.gov.au/F2021L00317/asmade/2021-03-24/text/original/epub/OEBPS/document_1/document_1.html#_Toc66194937"^^xsd:anyURI ;
    dcat:theme legcons:Item .

F2021L00317:181 a legcons:Item,
        owl:Class,
        dcat:Resource ;
    rdfs:label "Item - I181 8 18  Circumstances in which official mark must not be applied to fish or fish products"@en-AU ;
    dct:isPartOf F2021L00317:175 ;
    dct:isReferencedBy F2021L00317: ;
    rdfs:comment "8 18  Circumstances in which official mark must not be applied to fish or fish products - Abrievated Graph Key: I181"@en-AU ;
    skos:definition "8 18  Circumstances in which official mark must not be applied to fish or fish products"@en-AU ;
    skos:narrower F2021L00317:175 ;
    skos:prefLabel "Item I181"@en-AU ;
    dcat:accessURL <https://www.legislation.gov.au/F2021L00317/asmade/2021-03-24/text/original/epub/OEBPS/document_1/document_1.html#_Toc66194938> ;
    dcat:landingPage "https://www.legislation.gov.au/F2021L00317/asmade/2021-03-24/text/original/epub/OEBPS/document_1/document_1.html#_Toc66194938"^^xsd:anyURI ;
    dcat:theme legcons:Item .

F2021L00317:182 a legcons:Item,
        owl:Class,
        dcat:Resource ;
    rdfs:label "Item - I182 8 19  Alteration of and interference with official marks"@en-AU ;
    dct:isPartOf F2021L00317:175 ;
    dct:isReferencedBy F2021L00317: ;
    rdfs:comment "8 19  Alteration of and interference with official marks - Abrievated Graph Key: I182"@en-AU ;
    skos:definition "8 19  Alteration of and interference with official marks"@en-AU ;
    skos:narrower F2021L00317:175 ;
    skos:prefLabel "Item I182"@en-AU ;
    dcat:accessURL <https://www.legislation.gov.au/F2021L00317/asmade/2021-03-24/text/original/epub/OEBPS/document_1/document_1.html#_Toc66194939> ;
    dcat:landingPage "https://www.legislation.gov.au/F2021L00317/asmade/2021-03-24/text/original/epub/OEBPS/document_1/document_1.html#_Toc66194939"^^xsd:anyURI ;
    dcat:theme legcons:Item .

F2021L00317:183 a legcons:Item,
        owl:Class,
        dcat:Resource ;
    rdfs:label "Item - I183 8 20  Official marks must be legible and securely attached"@en-AU ;
    dct:isPartOf F2021L00317:175 ;
    dct:isReferencedBy F2021L00317: ;
    rdfs:comment "8 20  Official marks must be legible and securely attached - Abrievated Graph Key: I183"@en-AU ;
    skos:definition "8 20  Official marks must be legible and securely attached"@en-AU ;
    skos:narrower F2021L00317:175 ;
    skos:prefLabel "Item I183"@en-AU ;
    dcat:accessURL <https://www.legislation.gov.au/F2021L00317/asmade/2021-03-24/text/original/epub/OEBPS/document_1/document_1.html#_Toc66194940> ;
    dcat:landingPage "https://www.legislation.gov.au/F2021L00317/asmade/2021-03-24/text/original/epub/OEBPS/document_1/document_1.html#_Toc66194940"^^xsd:anyURI ;
    dcat:theme legcons:Item .

F2021L00317:184 a legcons:Item,
        owl:Class,
        dcat:Resource ;
    rdfs:label "Item - I184 8 21  Security of official marks"@en-AU ;
    dct:isPartOf F2021L00317:175 ;
    dct:isReferencedBy F2021L00317: ;
    rdfs:comment "8 21  Security of official marks - Abrievated Graph Key: I184"@en-AU ;
    skos:definition "8 21  Security of official marks"@en-AU ;
    skos:narrower F2021L00317:175 ;
    skos:prefLabel "Item I184"@en-AU ;
    dcat:accessURL <https://www.legislation.gov.au/F2021L00317/asmade/2021-03-24/text/original/epub/OEBPS/document_1/document_1.html#_Toc66194941> ;
    dcat:landingPage "https://www.legislation.gov.au/F2021L00317/asmade/2021-03-24/text/original/epub/OEBPS/document_1/document_1.html#_Toc66194941"^^xsd:anyURI ;
    dcat:theme legcons:Item .

F2021L00317:185 a legcons:Item,
        owl:Class,
        dcat:Resource ;
    rdfs:label "Item - I185 8 22  Removal or defacement of official marks"@en-AU ;
    dct:isPartOf F2021L00317:175 ;
    dct:isReferencedBy F2021L00317: ;
    rdfs:comment "8 22  Removal or defacement of official marks - Abrievated Graph Key: I185"@en-AU ;
    skos:definition "8 22  Removal or defacement of official marks"@en-AU ;
    skos:narrower F2021L00317:175 ;
    skos:prefLabel "Item I185"@en-AU ;
    dcat:accessURL <https://www.legislation.gov.au/F2021L00317/asmade/2021-03-24/text/original/epub/OEBPS/document_1/document_1.html#_Toc66194942> ;
    dcat:landingPage "https://www.legislation.gov.au/F2021L00317/asmade/2021-03-24/text/original/epub/OEBPS/document_1/document_1.html#_Toc66194942"^^xsd:anyURI ;
    dcat:theme legcons:Item .

F2021L00317:186 a legcons:Item,
        owl:Class,
        dcat:Resource ;
    rdfs:label "Item - I186 8 23  Records of official marks manufactured or supplied"@en-AU ;
    dct:isPartOf F2021L00317:175 ;
    dct:isReferencedBy F2021L00317: ;
    rdfs:comment "8 23  Records of official marks manufactured or supplied - Abrievated Graph Key: I186"@en-AU ;
    skos:definition "8 23  Records of official marks manufactured or supplied"@en-AU ;
    skos:narrower F2021L00317:175 ;
    skos:prefLabel "Item I186"@en-AU ;
    dcat:accessURL <https://www.legislation.gov.au/F2021L00317/asmade/2021-03-24/text/original/epub/OEBPS/document_1/document_1.html#_Toc66194943> ;
    dcat:landingPage "https://www.legislation.gov.au/F2021L00317/asmade/2021-03-24/text/original/epub/OEBPS/document_1/document_1.html#_Toc66194943"^^xsd:anyURI ;
    dcat:theme legcons:Item .

F2021L00317:187 a legcons:Item,
        owl:Class,
        dcat:Resource ;
    rdfs:label "Item - I187 8 24  Records of official marks received applied removed defaced destroyed or returned"@en-AU ;
    dct:isPartOf F2021L00317:175 ;
    dct:isReferencedBy F2021L00317: ;
    rdfs:comment "8 24  Records of official marks received applied removed defaced destroyed or returned - Abrievated Graph Key: I187"@en-AU ;
    skos:definition "8 24  Records of official marks received applied removed defaced destroyed or returned"@en-AU ;
    skos:narrower F2021L00317:175 ;
    skos:prefLabel "Item I187"@en-AU ;
    dcat:accessURL <https://www.legislation.gov.au/F2021L00317/asmade/2021-03-24/text/original/epub/OEBPS/document_1/document_1.html#_Toc66194944> ;
    dcat:landingPage "https://www.legislation.gov.au/F2021L00317/asmade/2021-03-24/text/original/epub/OEBPS/document_1/document_1.html#_Toc66194944"^^xsd:anyURI ;
    dcat:theme legcons:Item .

F2021L00317:189 a legcons:Item,
        owl:Class,
        dcat:Resource ;
    rdfs:label "Item - I189 8 25  Purpose of this Division"@en-AU ;
    dct:isPartOf F2021L00317:188 ;
    dct:isReferencedBy F2021L00317: ;
    rdfs:comment "8 25  Purpose of this Division - Abrievated Graph Key: I189"@en-AU ;
    skos:definition "8 25  Purpose of this Division"@en-AU ;
    skos:narrower F2021L00317:188 ;
    skos:prefLabel "Item I189"@en-AU ;
    dcat:accessURL <https://www.legislation.gov.au/F2021L00317/asmade/2021-03-24/text/original/epub/OEBPS/document_1/document_1.html#_Toc66194946> ;
    dcat:landingPage "https://www.legislation.gov.au/F2021L00317/asmade/2021-03-24/text/original/epub/OEBPS/document_1/document_1.html#_Toc66194946"^^xsd:anyURI ;
    dcat:theme legcons:Item .

F2021L00317:19 a legcons:Part,
        owl:Class,
        dcat:Resource ;
    rdfs:label "Part - P19 Part 2 Exemptions"@en-AU ;
    dct:isPartOf F2021L00317:11 ;
    dct:isReferencedBy F2021L00317: ;
    rdfs:comment "Part 2 Exemptions - Abrievated Graph Key: P19"@en-AU ;
    skos:definition "Part 2 Exemptions"@en-AU ;
    skos:narrower F2021L00317:11 ;
    skos:prefLabel "Part P19"@en-AU ;
    dcat:accessURL <https://www.legislation.gov.au/F2021L00317/asmade/2021-03-24/text/original/epub/OEBPS/document_1/document_1.html#_Toc66194776> ;
    dcat:landingPage "https://www.legislation.gov.au/F2021L00317/asmade/2021-03-24/text/original/epub/OEBPS/document_1/document_1.html#_Toc66194776"^^xsd:anyURI ;
    dcat:theme legcons:Part .

F2021L00317:190 a legcons:Item,
        owl:Class,
        dcat:Resource ;
    rdfs:label "Item - I190 8 26  Circumstances in which a mark resembles an official mark"@en-AU ;
    dct:isPartOf F2021L00317:188 ;
    dct:isReferencedBy F2021L00317: ;
    rdfs:comment "8 26  Circumstances in which a mark resembles an official mark - Abrievated Graph Key: I190"@en-AU ;
    skos:definition "8 26  Circumstances in which a mark resembles an official mark"@en-AU ;
    skos:narrower F2021L00317:188 ;
    skos:prefLabel "Item I190"@en-AU ;
    dcat:accessURL <https://www.legislation.gov.au/F2021L00317/asmade/2021-03-24/text/original/epub/OEBPS/document_1/document_1.html#_Toc66194947> ;
    dcat:landingPage "https://www.legislation.gov.au/F2021L00317/asmade/2021-03-24/text/original/epub/OEBPS/document_1/document_1.html#_Toc66194947"^^xsd:anyURI ;
    dcat:theme legcons:Item .

F2021L00317:191 a legcons:Item,
        owl:Class,
        dcat:Resource ;
    rdfs:label "Item - I191 8 27  Persons who may apply a resemblance"@en-AU ;
    dct:isPartOf F2021L00317:188 ;
    dct:isReferencedBy F2021L00317: ;
    rdfs:comment "8 27  Persons who may apply a resemblance - Abrievated Graph Key: I191"@en-AU ;
    skos:definition "8 27  Persons who may apply a resemblance"@en-AU ;
    skos:narrower F2021L00317:188 ;
    skos:prefLabel "Item I191"@en-AU ;
    dcat:accessURL <https://www.legislation.gov.au/F2021L00317/asmade/2021-03-24/text/original/epub/OEBPS/document_1/document_1.html#_Toc66194948> ;
    dcat:landingPage "https://www.legislation.gov.au/F2021L00317/asmade/2021-03-24/text/original/epub/OEBPS/document_1/document_1.html#_Toc66194948"^^xsd:anyURI ;
    dcat:theme legcons:Item .

F2021L00317:193 a legcons:Item,
        owl:Class,
        dcat:Resource ;
    rdfs:label "Item - I193 8 28  Purpose of this Division"@en-AU ;
    dct:isPartOf F2021L00317:192 ;
    dct:isReferencedBy F2021L00317: ;
    rdfs:comment "8 28  Purpose of this Division - Abrievated Graph Key: I193"@en-AU ;
    skos:definition "8 28  Purpose of this Division"@en-AU ;
    skos:narrower F2021L00317:192 ;
    skos:prefLabel "Item I193"@en-AU ;
    dcat:accessURL <https://www.legislation.gov.au/F2021L00317/asmade/2021-03-24/text/original/epub/OEBPS/document_1/document_1.html#_Toc66194950> ;
    dcat:landingPage "https://www.legislation.gov.au/F2021L00317/asmade/2021-03-24/text/original/epub/OEBPS/document_1/document_1.html#_Toc66194950"^^xsd:anyURI ;
    dcat:theme legcons:Item .

F2021L00317:194 a legcons:Item,
        owl:Class,
        dcat:Resource ;
    rdfs:label "Item - I194 8 29  Persons who may manufacture supply or possess official marking devices"@en-AU ;
    dct:isPartOf F2021L00317:192 ;
    dct:isReferencedBy F2021L00317: ;
    rdfs:comment "8 29  Persons who may manufacture supply or possess official marking devices - Abrievated Graph Key: I194"@en-AU ;
    skos:definition "8 29  Persons who may manufacture supply or possess official marking devices"@en-AU ;
    skos:narrower F2021L00317:192 ;
    skos:prefLabel "Item I194"@en-AU ;
    dcat:accessURL <https://www.legislation.gov.au/F2021L00317/asmade/2021-03-24/text/original/epub/OEBPS/document_1/document_1.html#_Toc66194951> ;
    dcat:landingPage "https://www.legislation.gov.au/F2021L00317/asmade/2021-03-24/text/original/epub/OEBPS/document_1/document_1.html#_Toc66194951"^^xsd:anyURI ;
    dcat:theme legcons:Item .

F2021L00317:195 a legcons:Item,
        owl:Class,
        dcat:Resource ;
    rdfs:label "Item - I195 8 30  Security of official marking devices"@en-AU ;
    dct:isPartOf F2021L00317:192 ;
    dct:isReferencedBy F2021L00317: ;
    rdfs:comment "8 30  Security of official marking devices - Abrievated Graph Key: I195"@en-AU ;
    skos:definition "8 30  Security of official marking devices"@en-AU ;
    skos:narrower F2021L00317:192 ;
    skos:prefLabel "Item I195"@en-AU ;
    dcat:accessURL <https://www.legislation.gov.au/F2021L00317/asmade/2021-03-24/text/original/epub/OEBPS/document_1/document_1.html#_Toc66194952> ;
    dcat:landingPage "https://www.legislation.gov.au/F2021L00317/asmade/2021-03-24/text/original/epub/OEBPS/document_1/document_1.html#_Toc66194952"^^xsd:anyURI ;
    dcat:theme legcons:Item .

F2021L00317:196 a legcons:Item,
        owl:Class,
        dcat:Resource ;
    rdfs:label "Item - I196 8 31  Damaged etc official marking devices"@en-AU ;
    dct:isPartOf F2021L00317:192 ;
    dct:isReferencedBy F2021L00317: ;
    rdfs:comment "8 31  Damaged etc official marking devices - Abrievated Graph Key: I196"@en-AU ;
    skos:definition "8 31  Damaged etc official marking devices"@en-AU ;
    skos:narrower F2021L00317:192 ;
    skos:prefLabel "Item I196"@en-AU ;
    dcat:accessURL <https://www.legislation.gov.au/F2021L00317/asmade/2021-03-24/text/original/epub/OEBPS/document_1/document_1.html#_Toc66194953> ;
    dcat:landingPage "https://www.legislation.gov.au/F2021L00317/asmade/2021-03-24/text/original/epub/OEBPS/document_1/document_1.html#_Toc66194953"^^xsd:anyURI ;
    dcat:theme legcons:Item .

F2021L00317:197 a legcons:Item,
        owl:Class,
        dcat:Resource ;
    rdfs:label "Item - I197 8 32  Records of official marking devices manufactured or supplied"@en-AU ;
    dct:isPartOf F2021L00317:192 ;
    dct:isReferencedBy F2021L00317: ;
    rdfs:comment "8 32  Records of official marking devices manufactured or supplied - Abrievated Graph Key: I197"@en-AU ;
    skos:definition "8 32  Records of official marking devices manufactured or supplied"@en-AU ;
    skos:narrower F2021L00317:192 ;
    skos:prefLabel "Item I197"@en-AU ;
    dcat:accessURL <https://www.legislation.gov.au/F2021L00317/asmade/2021-03-24/text/original/epub/OEBPS/document_1/document_1.html#_Toc66194954> ;
    dcat:landingPage "https://www.legislation.gov.au/F2021L00317/asmade/2021-03-24/text/original/epub/OEBPS/document_1/document_1.html#_Toc66194954"^^xsd:anyURI ;
    dcat:theme legcons:Item .

F2021L00317:198 a legcons:Item,
        owl:Class,
        dcat:Resource ;
    rdfs:label "Item - I198 8 33  Records of official marking devices received used damaged destroyed or returned"@en-AU ;
    dct:isPartOf F2021L00317:192 ;
    dct:isReferencedBy F2021L00317: ;
    rdfs:comment "8 33  Records of official marking devices received used damaged destroyed or returned - Abrievated Graph Key: I198"@en-AU ;
    skos:definition "8 33  Records of official marking devices received used damaged destroyed or returned"@en-AU ;
    skos:narrower F2021L00317:192 ;
    skos:prefLabel "Item I198"@en-AU ;
    dcat:accessURL <https://www.legislation.gov.au/F2021L00317/asmade/2021-03-24/text/original/epub/OEBPS/document_1/document_1.html#_Toc66194955> ;
    dcat:landingPage "https://www.legislation.gov.au/F2021L00317/asmade/2021-03-24/text/original/epub/OEBPS/document_1/document_1.html#_Toc66194955"^^xsd:anyURI ;
    dcat:theme legcons:Item .

F2021L00317:2 a legcons:Part,
        owl:Class,
        dcat:Resource ;
    rdfs:label "Part - P2 Part 1 Preliminary"@en-AU ;
    dct:isPartOf F2021L00317:1 ;
    dct:isReferencedBy F2021L00317: ;
    rdfs:comment "Part 1 Preliminary - Abrievated Graph Key: P2"@en-AU ;
    skos:definition "Part 1 Preliminary"@en-AU ;
    skos:narrower F2021L00317:1 ;
    skos:prefLabel "Part P2"@en-AU ;
    dcat:accessURL <https://www.legislation.gov.au/F2021L00317/asmade/2021-03-24/text/original/epub/OEBPS/document_1/document_1.html#_Toc66194759> ;
    dcat:landingPage "https://www.legislation.gov.au/F2021L00317/asmade/2021-03-24/text/original/epub/OEBPS/document_1/document_1.html#_Toc66194759"^^xsd:anyURI ;
    dcat:theme legcons:Part .

F2021L00317:20 a legcons:Item,
        owl:Class,
        dcat:Resource ;
    rdfs:label "Item - I20 2 5  Application of this Part"@en-AU ;
    dct:isPartOf F2021L00317:11 ;
    dct:isReferencedBy F2021L00317: ;
    rdfs:comment "2 5  Application of this Part - Abrievated Graph Key: I20"@en-AU ;
    skos:definition "2 5  Application of this Part"@en-AU ;
    skos:narrower F2021L00317:11 ;
    skos:prefLabel "Item I20"@en-AU ;
    dcat:accessURL <https://www.legislation.gov.au/F2021L00317/asmade/2021-03-24/text/original/epub/OEBPS/document_1/document_1.html#_Toc66194777> ;
    dcat:landingPage "https://www.legislation.gov.au/F2021L00317/asmade/2021-03-24/text/original/epub/OEBPS/document_1/document_1.html#_Toc66194777"^^xsd:anyURI ;
    dcat:theme legcons:Item .

F2021L00317:202 a legcons:Item,
        owl:Class,
        dcat:Resource ;
    rdfs:label "Item - I202 9 1  References to audit in this Part"@en-AU ;
    dct:isPartOf F2021L00317:201 ;
    dct:isReferencedBy F2021L00317: ;
    rdfs:comment "9 1  References to audit in this Part - Abrievated Graph Key: I202"@en-AU ;
    skos:definition "9 1  References to audit in this Part"@en-AU ;
    skos:narrower F2021L00317:201 ;
    skos:prefLabel "Item I202"@en-AU ;
    dcat:accessURL <https://www.legislation.gov.au/F2021L00317/asmade/2021-03-24/text/original/epub/OEBPS/document_1/document_1.html#_Toc66194959> ;
    dcat:landingPage "https://www.legislation.gov.au/F2021L00317/asmade/2021-03-24/text/original/epub/OEBPS/document_1/document_1.html#_Toc66194959"^^xsd:anyURI ;
    dcat:theme legcons:Item .

F2021L00317:203 a legcons:Item,
        owl:Class,
        dcat:Resource ;
    rdfs:label "Item - I203 9 2  Audits of export operations"@en-AU ;
    dct:isPartOf F2021L00317:201 ;
    dct:isReferencedBy F2021L00317: ;
    rdfs:comment "9 2  Audits of export operations - Abrievated Graph Key: I203"@en-AU ;
    skos:definition "9 2  Audits of export operations"@en-AU ;
    skos:narrower F2021L00317:201 ;
    skos:prefLabel "Item I203"@en-AU ;
    dcat:accessURL <https://www.legislation.gov.au/F2021L00317/asmade/2021-03-24/text/original/epub/OEBPS/document_1/document_1.html#_Toc66194960> ;
    dcat:landingPage "https://www.legislation.gov.au/F2021L00317/asmade/2021-03-24/text/original/epub/OEBPS/document_1/document_1.html#_Toc66194960"^^xsd:anyURI ;
    dcat:theme legcons:Item .

F2021L00317:205 a legcons:Item,
        owl:Class,
        dcat:Resource ;
    rdfs:label "Item - I205 9 3  Purpose of this Division"@en-AU ;
    dct:isPartOf F2021L00317:204 ;
    dct:isReferencedBy F2021L00317: ;
    rdfs:comment "9 3  Purpose of this Division - Abrievated Graph Key: I205"@en-AU ;
    skos:definition "9 3  Purpose of this Division"@en-AU ;
    skos:narrower F2021L00317:204 ;
    skos:prefLabel "Item I205"@en-AU ;
    dcat:accessURL <https://www.legislation.gov.au/F2021L00317/asmade/2021-03-24/text/original/epub/OEBPS/document_1/document_1.html#_Toc66194962> ;
    dcat:landingPage "https://www.legislation.gov.au/F2021L00317/asmade/2021-03-24/text/original/epub/OEBPS/document_1/document_1.html#_Toc66194962"^^xsd:anyURI ;
    dcat:theme legcons:Item .

F2021L00317:206 a legcons:Item,
        owl:Class,
        dcat:Resource ;
    rdfs:label "Item - I206 9 4  Manner in which audit must be conducted"@en-AU ;
    dct:isPartOf F2021L00317:204 ;
    dct:isReferencedBy F2021L00317: ;
    rdfs:comment "9 4  Manner in which audit must be conducted - Abrievated Graph Key: I206"@en-AU ;
    skos:definition "9 4  Manner in which audit must be conducted"@en-AU ;
    skos:narrower F2021L00317:204 ;
    skos:prefLabel "Item I206"@en-AU ;
    dcat:accessURL <https://www.legislation.gov.au/F2021L00317/asmade/2021-03-24/text/original/epub/OEBPS/document_1/document_1.html#_Toc66194963> ;
    dcat:landingPage "https://www.legislation.gov.au/F2021L00317/asmade/2021-03-24/text/original/epub/OEBPS/document_1/document_1.html#_Toc66194963"^^xsd:anyURI ;
    dcat:theme legcons:Item .

F2021L00317:207 a legcons:Item,
        owl:Class,
        dcat:Resource ;
    rdfs:label "Item - I207 9 5  Notice of non compliance with requirements"@en-AU ;
    dct:isPartOf F2021L00317:204 ;
    dct:isReferencedBy F2021L00317: ;
    rdfs:comment "9 5  Notice of non compliance with requirements - Abrievated Graph Key: I207"@en-AU ;
    skos:definition "9 5  Notice of non compliance with requirements"@en-AU ;
    skos:narrower F2021L00317:204 ;
    skos:prefLabel "Item I207"@en-AU ;
    dcat:accessURL <https://www.legislation.gov.au/F2021L00317/asmade/2021-03-24/text/original/epub/OEBPS/document_1/document_1.html#_Toc66194964> ;
    dcat:landingPage "https://www.legislation.gov.au/F2021L00317/asmade/2021-03-24/text/original/epub/OEBPS/document_1/document_1.html#_Toc66194964"^^xsd:anyURI ;
    dcat:theme legcons:Item .

F2021L00317:208 a legcons:Item,
        owl:Class,
        dcat:Resource ;
    rdfs:label "Item - I208 9 6  Audit reports"@en-AU ;
    dct:isPartOf F2021L00317:204 ;
    dct:isReferencedBy F2021L00317: ;
    rdfs:comment "9 6  Audit reports - Abrievated Graph Key: I208"@en-AU ;
    skos:definition "9 6  Audit reports"@en-AU ;
    skos:narrower F2021L00317:204 ;
    skos:prefLabel "Item I208"@en-AU ;
    dcat:accessURL <https://www.legislation.gov.au/F2021L00317/asmade/2021-03-24/text/original/epub/OEBPS/document_1/document_1.html#_Toc66194965> ;
    dcat:landingPage "https://www.legislation.gov.au/F2021L00317/asmade/2021-03-24/text/original/epub/OEBPS/document_1/document_1.html#_Toc66194965"^^xsd:anyURI ;
    dcat:theme legcons:Item .

F2021L00317:21 a legcons:Item,
        owl:Class,
        dcat:Resource ;
    rdfs:label "Item - I21 2 6  Prescribed circumstancetesting the market"@en-AU ;
    dct:isPartOf F2021L00317:11 ;
    dct:isReferencedBy F2021L00317: ;
    rdfs:comment "2 6  Prescribed circumstancetesting the market - Abrievated Graph Key: I21"@en-AU ;
    skos:definition "2 6  Prescribed circumstancetesting the market"@en-AU ;
    skos:narrower F2021L00317:11 ;
    skos:prefLabel "Item I21"@en-AU ;
    dcat:accessURL <https://www.legislation.gov.au/F2021L00317/asmade/2021-03-24/text/original/epub/OEBPS/document_1/document_1.html#_Toc66194778> ;
    dcat:landingPage "https://www.legislation.gov.au/F2021L00317/asmade/2021-03-24/text/original/epub/OEBPS/document_1/document_1.html#_Toc66194778"^^xsd:anyURI ;
    dcat:theme legcons:Item .

F2021L00317:210 a legcons:Item,
        owl:Class,
        dcat:Resource ;
    rdfs:label "Item - I210 9 7  Purpose of this Division"@en-AU ;
    dct:isPartOf F2021L00317:209 ;
    dct:isReferencedBy F2021L00317: ;
    rdfs:comment "9 7  Purpose of this Division - Abrievated Graph Key: I210"@en-AU ;
    skos:definition "9 7  Purpose of this Division"@en-AU ;
    skos:narrower F2021L00317:209 ;
    skos:prefLabel "Item I210"@en-AU ;
    dcat:accessURL <https://www.legislation.gov.au/F2021L00317/asmade/2021-03-24/text/original/epub/OEBPS/document_1/document_1.html#_Toc66194967> ;
    dcat:landingPage "https://www.legislation.gov.au/F2021L00317/asmade/2021-03-24/text/original/epub/OEBPS/document_1/document_1.html#_Toc66194967"^^xsd:anyURI ;
    dcat:theme legcons:Item .

F2021L00317:211 a legcons:Item,
        owl:Class,
        dcat:Resource ;
    rdfs:label "Item - I211 9 8  Application for approval"@en-AU ;
    dct:isPartOf F2021L00317:209 ;
    dct:isReferencedBy F2021L00317: ;
    rdfs:comment "9 8  Application for approval - Abrievated Graph Key: I211"@en-AU ;
    skos:definition "9 8  Application for approval"@en-AU ;
    skos:narrower F2021L00317:209 ;
    skos:prefLabel "Item I211"@en-AU ;
    dcat:accessURL <https://www.legislation.gov.au/F2021L00317/asmade/2021-03-24/text/original/epub/OEBPS/document_1/document_1.html#_Toc66194968> ;
    dcat:landingPage "https://www.legislation.gov.au/F2021L00317/asmade/2021-03-24/text/original/epub/OEBPS/document_1/document_1.html#_Toc66194968"^^xsd:anyURI ;
    dcat:theme legcons:Item .

F2021L00317:212 a legcons:Item,
        owl:Class,
        dcat:Resource ;
    rdfs:label "Item - I212 9 9  Secretary must decide whether to approve applicant to conduct audits"@en-AU ;
    dct:isPartOf F2021L00317:209 ;
    dct:isReferencedBy F2021L00317: ;
    rdfs:comment "9 9  Secretary must decide whether to approve applicant to conduct audits - Abrievated Graph Key: I212"@en-AU ;
    skos:definition "9 9  Secretary must decide whether to approve applicant to conduct audits"@en-AU ;
    skos:narrower F2021L00317:209 ;
    skos:prefLabel "Item I212"@en-AU ;
    dcat:accessURL <https://www.legislation.gov.au/F2021L00317/asmade/2021-03-24/text/original/epub/OEBPS/document_1/document_1.html#_Toc66194969> ;
    dcat:landingPage "https://www.legislation.gov.au/F2021L00317/asmade/2021-03-24/text/original/epub/OEBPS/document_1/document_1.html#_Toc66194969"^^xsd:anyURI ;
    dcat:theme legcons:Item .

F2021L00317:213 a legcons:Item,
        owl:Class,
        dcat:Resource ;
    rdfs:label "Item - I213 9 10  Dealing with applications"@en-AU ;
    dct:isPartOf F2021L00317:209 ;
    dct:isReferencedBy F2021L00317: ;
    rdfs:comment "9 10  Dealing with applications - Abrievated Graph Key: I213"@en-AU ;
    skos:definition "9 10  Dealing with applications"@en-AU ;
    skos:narrower F2021L00317:209 ;
    skos:prefLabel "Item I213"@en-AU ;
    dcat:accessURL <https://www.legislation.gov.au/F2021L00317/asmade/2021-03-24/text/original/epub/OEBPS/document_1/document_1.html#_Toc66194970> ;
    dcat:landingPage "https://www.legislation.gov.au/F2021L00317/asmade/2021-03-24/text/original/epub/OEBPS/document_1/document_1.html#_Toc66194970"^^xsd:anyURI ;
    dcat:theme legcons:Item .

F2021L00317:214 a legcons:Item,
        owl:Class,
        dcat:Resource ;
    rdfs:label "Item - I214 9 11  Conditions of approval"@en-AU ;
    dct:isPartOf F2021L00317:209 ;
    dct:isReferencedBy F2021L00317: ;
    rdfs:comment "9 11  Conditions of approval - Abrievated Graph Key: I214"@en-AU ;
    skos:definition "9 11  Conditions of approval"@en-AU ;
    skos:narrower F2021L00317:209 ;
    skos:prefLabel "Item I214"@en-AU ;
    dcat:accessURL <https://www.legislation.gov.au/F2021L00317/asmade/2021-03-24/text/original/epub/OEBPS/document_1/document_1.html#_Toc66194971> ;
    dcat:landingPage "https://www.legislation.gov.au/F2021L00317/asmade/2021-03-24/text/original/epub/OEBPS/document_1/document_1.html#_Toc66194971"^^xsd:anyURI ;
    dcat:theme legcons:Item .

F2021L00317:215 a legcons:Item,
        owl:Class,
        dcat:Resource ;
    rdfs:label "Item - I215 9 12  Notice of decision"@en-AU ;
    dct:isPartOf F2021L00317:209 ;
    dct:isReferencedBy F2021L00317: ;
    rdfs:comment "9 12  Notice of decision - Abrievated Graph Key: I215"@en-AU ;
    skos:definition "9 12  Notice of decision"@en-AU ;
    skos:narrower F2021L00317:209 ;
    skos:prefLabel "Item I215"@en-AU ;
    dcat:accessURL <https://www.legislation.gov.au/F2021L00317/asmade/2021-03-24/text/original/epub/OEBPS/document_1/document_1.html#_Toc66194972> ;
    dcat:landingPage "https://www.legislation.gov.au/F2021L00317/asmade/2021-03-24/text/original/epub/OEBPS/document_1/document_1.html#_Toc66194972"^^xsd:anyURI ;
    dcat:theme legcons:Item .

F2021L00317:216 a legcons:Item,
        owl:Class,
        dcat:Resource ;
    rdfs:label "Item - I216 9 13  Period of effect of approval"@en-AU ;
    dct:isPartOf F2021L00317:209 ;
    dct:isReferencedBy F2021L00317: ;
    rdfs:comment "9 13  Period of effect of approval - Abrievated Graph Key: I216"@en-AU ;
    skos:definition "9 13  Period of effect of approval"@en-AU ;
    skos:narrower F2021L00317:209 ;
    skos:prefLabel "Item I216"@en-AU ;
    dcat:accessURL <https://www.legislation.gov.au/F2021L00317/asmade/2021-03-24/text/original/epub/OEBPS/document_1/document_1.html#_Toc66194973> ;
    dcat:landingPage "https://www.legislation.gov.au/F2021L00317/asmade/2021-03-24/text/original/epub/OEBPS/document_1/document_1.html#_Toc66194973"^^xsd:anyURI ;
    dcat:theme legcons:Item .

F2021L00317:217 a legcons:Item,
        owl:Class,
        dcat:Resource ;
    rdfs:label "Item - I217 9 14  Imposing or varying conditions of approval"@en-AU ;
    dct:isPartOf F2021L00317:209 ;
    dct:isReferencedBy F2021L00317: ;
    rdfs:comment "9 14  Imposing or varying conditions of approval - Abrievated Graph Key: I217"@en-AU ;
    skos:definition "9 14  Imposing or varying conditions of approval"@en-AU ;
    skos:narrower F2021L00317:209 ;
    skos:prefLabel "Item I217"@en-AU ;
    dcat:accessURL <https://www.legislation.gov.au/F2021L00317/asmade/2021-03-24/text/original/epub/OEBPS/document_1/document_1.html#_Toc66194974> ;
    dcat:landingPage "https://www.legislation.gov.au/F2021L00317/asmade/2021-03-24/text/original/epub/OEBPS/document_1/document_1.html#_Toc66194974"^^xsd:anyURI ;
    dcat:theme legcons:Item .

F2021L00317:218 a legcons:Item,
        owl:Class,
        dcat:Resource ;
    rdfs:label "Item - I218 9 15  Revocation of approval"@en-AU ;
    dct:isPartOf F2021L00317:209 ;
    dct:isReferencedBy F2021L00317: ;
    rdfs:comment "9 15  Revocation of approval - Abrievated Graph Key: I218"@en-AU ;
    skos:definition "9 15  Revocation of approval"@en-AU ;
    skos:narrower F2021L00317:209 ;
    skos:prefLabel "Item I218"@en-AU ;
    dcat:accessURL <https://www.legislation.gov.au/F2021L00317/asmade/2021-03-24/text/original/epub/OEBPS/document_1/document_1.html#_Toc66194975> ;
    dcat:landingPage "https://www.legislation.gov.au/F2021L00317/asmade/2021-03-24/text/original/epub/OEBPS/document_1/document_1.html#_Toc66194975"^^xsd:anyURI ;
    dcat:theme legcons:Item .

F2021L00317:219 a legcons:Item,
        owl:Class,
        dcat:Resource ;
    rdfs:label "Item - I219 9 16  Register of approved auditors"@en-AU ;
    dct:isPartOf F2021L00317:209 ;
    dct:isReferencedBy F2021L00317: ;
    rdfs:comment "9 16  Register of approved auditors - Abrievated Graph Key: I219"@en-AU ;
    skos:definition "9 16  Register of approved auditors"@en-AU ;
    skos:narrower F2021L00317:209 ;
    skos:prefLabel "Item I219"@en-AU ;
    dcat:accessURL <https://www.legislation.gov.au/F2021L00317/asmade/2021-03-24/text/original/epub/OEBPS/document_1/document_1.html#_Toc66194976> ;
    dcat:landingPage "https://www.legislation.gov.au/F2021L00317/asmade/2021-03-24/text/original/epub/OEBPS/document_1/document_1.html#_Toc66194976"^^xsd:anyURI ;
    dcat:theme legcons:Item .

F2021L00317:22 a legcons:Item,
        owl:Class,
        dcat:Resource ;
    rdfs:label "Item - I22 2 7  Prescribed meaningcommercial sample"@en-AU ;
    dct:isPartOf F2021L00317:11 ;
    dct:isReferencedBy F2021L00317: ;
    rdfs:comment "2 7  Prescribed meaningcommercial sample - Abrievated Graph Key: I22"@en-AU ;
    skos:definition "2 7  Prescribed meaningcommercial sample"@en-AU ;
    skos:narrower F2021L00317:11 ;
    skos:prefLabel "Item I22"@en-AU ;
    dcat:accessURL <https://www.legislation.gov.au/F2021L00317/asmade/2021-03-24/text/original/epub/OEBPS/document_1/document_1.html#_Toc66194779> ;
    dcat:landingPage "https://www.legislation.gov.au/F2021L00317/asmade/2021-03-24/text/original/epub/OEBPS/document_1/document_1.html#_Toc66194779"^^xsd:anyURI ;
    dcat:theme legcons:Item .

F2021L00317:220 a legcons:Item,
        owl:Class,
        dcat:Resource ;
    rdfs:label "Item - I220 9 17  Fit and proper person test"@en-AU ;
    dct:isPartOf F2021L00317:209 ;
    dct:isReferencedBy F2021L00317: ;
    rdfs:comment "9 17  Fit and proper person test - Abrievated Graph Key: I220"@en-AU ;
    skos:definition "9 17  Fit and proper person test"@en-AU ;
    skos:narrower F2021L00317:209 ;
    skos:prefLabel "Item I220"@en-AU ;
    dcat:accessURL <https://www.legislation.gov.au/F2021L00317/asmade/2021-03-24/text/original/epub/OEBPS/document_1/document_1.html#_Toc66194977> ;
    dcat:landingPage "https://www.legislation.gov.au/F2021L00317/asmade/2021-03-24/text/original/epub/OEBPS/document_1/document_1.html#_Toc66194977"^^xsd:anyURI ;
    dcat:theme legcons:Item .

F2021L00317:223 a legcons:Item,
        owl:Class,
        dcat:Resource ;
    rdfs:label "Item - I223 9 18  References to assessment in this Part"@en-AU ;
    dct:isPartOf F2021L00317:222 ;
    dct:isReferencedBy F2021L00317: ;
    rdfs:comment "9 18  References to assessment in this Part - Abrievated Graph Key: I223"@en-AU ;
    skos:definition "9 18  References to assessment in this Part"@en-AU ;
    skos:narrower F2021L00317:222 ;
    skos:prefLabel "Item I223"@en-AU ;
    dcat:accessURL <https://www.legislation.gov.au/F2021L00317/asmade/2021-03-24/text/original/epub/OEBPS/document_1/document_1.html#_Toc66194980> ;
    dcat:landingPage "https://www.legislation.gov.au/F2021L00317/asmade/2021-03-24/text/original/epub/OEBPS/document_1/document_1.html#_Toc66194980"^^xsd:anyURI ;
    dcat:theme legcons:Item .

F2021L00317:225 a legcons:Item,
        owl:Class,
        dcat:Resource ;
    rdfs:label "Item - I225 9 19  Circumstances in which assessment may be required or permitted"@en-AU ;
    dct:isPartOf F2021L00317:224 ;
    dct:isReferencedBy F2021L00317: ;
    rdfs:comment "9 19  Circumstances in which assessment may be required or permitted - Abrievated Graph Key: I225"@en-AU ;
    skos:definition "9 19  Circumstances in which assessment may be required or permitted"@en-AU ;
    skos:narrower F2021L00317:224 ;
    skos:prefLabel "Item I225"@en-AU ;
    dcat:accessURL <https://www.legislation.gov.au/F2021L00317/asmade/2021-03-24/text/original/epub/OEBPS/document_1/document_1.html#_Toc66194982> ;
    dcat:landingPage "https://www.legislation.gov.au/F2021L00317/asmade/2021-03-24/text/original/epub/OEBPS/document_1/document_1.html#_Toc66194982"^^xsd:anyURI ;
    dcat:theme legcons:Item .

F2021L00317:226 a legcons:Item,
        owl:Class,
        dcat:Resource ;
    rdfs:label "Item - I226 9 20  Process to be followed after assessment completed"@en-AU ;
    dct:isPartOf F2021L00317:224 ;
    dct:isReferencedBy F2021L00317: ;
    rdfs:comment "9 20  Process to be followed after assessment completed - Abrievated Graph Key: I226"@en-AU ;
    skos:definition "9 20  Process to be followed after assessment completed"@en-AU ;
    skos:narrower F2021L00317:224 ;
    skos:prefLabel "Item I226"@en-AU ;
    dcat:accessURL <https://www.legislation.gov.au/F2021L00317/asmade/2021-03-24/text/original/epub/OEBPS/document_1/document_1.html#_Toc66194983> ;
    dcat:landingPage "https://www.legislation.gov.au/F2021L00317/asmade/2021-03-24/text/original/epub/OEBPS/document_1/document_1.html#_Toc66194983"^^xsd:anyURI ;
    dcat:theme legcons:Item .

F2021L00317:228 a legcons:Item,
        owl:Class,
        dcat:Resource ;
    rdfs:label "Item - I228 9 21  Purpose of this Division"@en-AU ;
    dct:isPartOf F2021L00317:227 ;
    dct:isReferencedBy F2021L00317: ;
    rdfs:comment "9 21  Purpose of this Division - Abrievated Graph Key: I228"@en-AU ;
    skos:definition "9 21  Purpose of this Division"@en-AU ;
    skos:narrower F2021L00317:227 ;
    skos:prefLabel "Item I228"@en-AU ;
    dcat:accessURL <https://www.legislation.gov.au/F2021L00317/asmade/2021-03-24/text/original/epub/OEBPS/document_1/document_1.html#_Toc66194985> ;
    dcat:landingPage "https://www.legislation.gov.au/F2021L00317/asmade/2021-03-24/text/original/epub/OEBPS/document_1/document_1.html#_Toc66194985"^^xsd:anyURI ;
    dcat:theme legcons:Item .

F2021L00317:229 a legcons:Item,
        owl:Class,
        dcat:Resource ;
    rdfs:label "Item - I229 9 22  Application for approval"@en-AU ;
    dct:isPartOf F2021L00317:227 ;
    dct:isReferencedBy F2021L00317: ;
    rdfs:comment "9 22  Application for approval - Abrievated Graph Key: I229"@en-AU ;
    skos:definition "9 22  Application for approval"@en-AU ;
    skos:narrower F2021L00317:227 ;
    skos:prefLabel "Item I229"@en-AU ;
    dcat:accessURL <https://www.legislation.gov.au/F2021L00317/asmade/2021-03-24/text/original/epub/OEBPS/document_1/document_1.html#_Toc66194986> ;
    dcat:landingPage "https://www.legislation.gov.au/F2021L00317/asmade/2021-03-24/text/original/epub/OEBPS/document_1/document_1.html#_Toc66194986"^^xsd:anyURI ;
    dcat:theme legcons:Item .

F2021L00317:23 a legcons:Item,
        owl:Class,
        dcat:Resource ;
    rdfs:label "Item - I23 2 8  Period for making application for exemption"@en-AU ;
    dct:isPartOf F2021L00317:11 ;
    dct:isReferencedBy F2021L00317: ;
    rdfs:comment "2 8  Period for making application for exemption - Abrievated Graph Key: I23"@en-AU ;
    skos:definition "2 8  Period for making application for exemption"@en-AU ;
    skos:narrower F2021L00317:11 ;
    skos:prefLabel "Item I23"@en-AU ;
    dcat:accessURL <https://www.legislation.gov.au/F2021L00317/asmade/2021-03-24/text/original/epub/OEBPS/document_1/document_1.html#_Toc66194780> ;
    dcat:landingPage "https://www.legislation.gov.au/F2021L00317/asmade/2021-03-24/text/original/epub/OEBPS/document_1/document_1.html#_Toc66194780"^^xsd:anyURI ;
    dcat:theme legcons:Item .

F2021L00317:230 a legcons:Item,
        owl:Class,
        dcat:Resource ;
    rdfs:label "Item - I230 9 23  Secretary must decide whether to approve applicant to carry out assessments"@en-AU ;
    dct:isPartOf F2021L00317:227 ;
    dct:isReferencedBy F2021L00317: ;
    rdfs:comment "9 23  Secretary must decide whether to approve applicant to carry out assessments - Abrievated Graph Key: I230"@en-AU ;
    skos:definition "9 23  Secretary must decide whether to approve applicant to carry out assessments"@en-AU ;
    skos:narrower F2021L00317:227 ;
    skos:prefLabel "Item I230"@en-AU ;
    dcat:accessURL <https://www.legislation.gov.au/F2021L00317/asmade/2021-03-24/text/original/epub/OEBPS/document_1/document_1.html#_Toc66194987> ;
    dcat:landingPage "https://www.legislation.gov.au/F2021L00317/asmade/2021-03-24/text/original/epub/OEBPS/document_1/document_1.html#_Toc66194987"^^xsd:anyURI ;
    dcat:theme legcons:Item .

F2021L00317:231 a legcons:Item,
        owl:Class,
        dcat:Resource ;
    rdfs:label "Item - I231 9 24  Dealing with applications"@en-AU ;
    dct:isPartOf F2021L00317:227 ;
    dct:isReferencedBy F2021L00317: ;
    rdfs:comment "9 24  Dealing with applications - Abrievated Graph Key: I231"@en-AU ;
    skos:definition "9 24  Dealing with applications"@en-AU ;
    skos:narrower F2021L00317:227 ;
    skos:prefLabel "Item I231"@en-AU ;
    dcat:accessURL <https://www.legislation.gov.au/F2021L00317/asmade/2021-03-24/text/original/epub/OEBPS/document_1/document_1.html#_Toc66194988> ;
    dcat:landingPage "https://www.legislation.gov.au/F2021L00317/asmade/2021-03-24/text/original/epub/OEBPS/document_1/document_1.html#_Toc66194988"^^xsd:anyURI ;
    dcat:theme legcons:Item .

F2021L00317:232 a legcons:Item,
        owl:Class,
        dcat:Resource ;
    rdfs:label "Item - I232 9 25  Conditions of approval"@en-AU ;
    dct:isPartOf F2021L00317:227 ;
    dct:isReferencedBy F2021L00317: ;
    rdfs:comment "9 25  Conditions of approval - Abrievated Graph Key: I232"@en-AU ;
    skos:definition "9 25  Conditions of approval"@en-AU ;
    skos:narrower F2021L00317:227 ;
    skos:prefLabel "Item I232"@en-AU ;
    dcat:accessURL <https://www.legislation.gov.au/F2021L00317/asmade/2021-03-24/text/original/epub/OEBPS/document_1/document_1.html#_Toc66194989> ;
    dcat:landingPage "https://www.legislation.gov.au/F2021L00317/asmade/2021-03-24/text/original/epub/OEBPS/document_1/document_1.html#_Toc66194989"^^xsd:anyURI ;
    dcat:theme legcons:Item .

F2021L00317:233 a legcons:Item,
        owl:Class,
        dcat:Resource ;
    rdfs:label "Item - I233 9 26  Notice of decision"@en-AU ;
    dct:isPartOf F2021L00317:227 ;
    dct:isReferencedBy F2021L00317: ;
    rdfs:comment "9 26  Notice of decision - Abrievated Graph Key: I233"@en-AU ;
    skos:definition "9 26  Notice of decision"@en-AU ;
    skos:narrower F2021L00317:227 ;
    skos:prefLabel "Item I233"@en-AU ;
    dcat:accessURL <https://www.legislation.gov.au/F2021L00317/asmade/2021-03-24/text/original/epub/OEBPS/document_1/document_1.html#_Toc66194990> ;
    dcat:landingPage "https://www.legislation.gov.au/F2021L00317/asmade/2021-03-24/text/original/epub/OEBPS/document_1/document_1.html#_Toc66194990"^^xsd:anyURI ;
    dcat:theme legcons:Item .

F2021L00317:234 a legcons:Item,
        owl:Class,
        dcat:Resource ;
    rdfs:label "Item - I234 9 27  Period of effect of approval"@en-AU ;
    dct:isPartOf F2021L00317:227 ;
    dct:isReferencedBy F2021L00317: ;
    rdfs:comment "9 27  Period of effect of approval - Abrievated Graph Key: I234"@en-AU ;
    skos:definition "9 27  Period of effect of approval"@en-AU ;
    skos:narrower F2021L00317:227 ;
    skos:prefLabel "Item I234"@en-AU ;
    dcat:accessURL <https://www.legislation.gov.au/F2021L00317/asmade/2021-03-24/text/original/epub/OEBPS/document_1/document_1.html#_Toc66194991> ;
    dcat:landingPage "https://www.legislation.gov.au/F2021L00317/asmade/2021-03-24/text/original/epub/OEBPS/document_1/document_1.html#_Toc66194991"^^xsd:anyURI ;
    dcat:theme legcons:Item .

F2021L00317:235 a legcons:Item,
        owl:Class,
        dcat:Resource ;
    rdfs:label "Item - I235 9 28  Imposing or varying conditions of approval"@en-AU ;
    dct:isPartOf F2021L00317:227 ;
    dct:isReferencedBy F2021L00317: ;
    rdfs:comment "9 28  Imposing or varying conditions of approval - Abrievated Graph Key: I235"@en-AU ;
    skos:definition "9 28  Imposing or varying conditions of approval"@en-AU ;
    skos:narrower F2021L00317:227 ;
    skos:prefLabel "Item I235"@en-AU ;
    dcat:accessURL <https://www.legislation.gov.au/F2021L00317/asmade/2021-03-24/text/original/epub/OEBPS/document_1/document_1.html#_Toc66194992> ;
    dcat:landingPage "https://www.legislation.gov.au/F2021L00317/asmade/2021-03-24/text/original/epub/OEBPS/document_1/document_1.html#_Toc66194992"^^xsd:anyURI ;
    dcat:theme legcons:Item .

F2021L00317:236 a legcons:Item,
        owl:Class,
        dcat:Resource ;
    rdfs:label "Item - I236 9 29  Revocation of approval"@en-AU ;
    dct:isPartOf F2021L00317:227 ;
    dct:isReferencedBy F2021L00317: ;
    rdfs:comment "9 29  Revocation of approval - Abrievated Graph Key: I236"@en-AU ;
    skos:definition "9 29  Revocation of approval"@en-AU ;
    skos:narrower F2021L00317:227 ;
    skos:prefLabel "Item I236"@en-AU ;
    dcat:accessURL <https://www.legislation.gov.au/F2021L00317/asmade/2021-03-24/text/original/epub/OEBPS/document_1/document_1.html#_Toc66194993> ;
    dcat:landingPage "https://www.legislation.gov.au/F2021L00317/asmade/2021-03-24/text/original/epub/OEBPS/document_1/document_1.html#_Toc66194993"^^xsd:anyURI ;
    dcat:theme legcons:Item .

F2021L00317:237 a legcons:Item,
        owl:Class,
        dcat:Resource ;
    rdfs:label "Item - I237 9 30  Register of approved assessors"@en-AU ;
    dct:isPartOf F2021L00317:227 ;
    dct:isReferencedBy F2021L00317: ;
    rdfs:comment "9 30  Register of approved assessors - Abrievated Graph Key: I237"@en-AU ;
    skos:definition "9 30  Register of approved assessors"@en-AU ;
    skos:narrower F2021L00317:227 ;
    skos:prefLabel "Item I237"@en-AU ;
    dcat:accessURL <https://www.legislation.gov.au/F2021L00317/asmade/2021-03-24/text/original/epub/OEBPS/document_1/document_1.html#_Toc66194994> ;
    dcat:landingPage "https://www.legislation.gov.au/F2021L00317/asmade/2021-03-24/text/original/epub/OEBPS/document_1/document_1.html#_Toc66194994"^^xsd:anyURI ;
    dcat:theme legcons:Item .

F2021L00317:238 a legcons:Item,
        owl:Class,
        dcat:Resource ;
    rdfs:label "Item - I238 9 31  Fit and proper person test"@en-AU ;
    dct:isPartOf F2021L00317:227 ;
    dct:isReferencedBy F2021L00317: ;
    rdfs:comment "9 31  Fit and proper person test - Abrievated Graph Key: I238"@en-AU ;
    skos:definition "9 31  Fit and proper person test"@en-AU ;
    skos:narrower F2021L00317:227 ;
    skos:prefLabel "Item I238"@en-AU ;
    dcat:accessURL <https://www.legislation.gov.au/F2021L00317/asmade/2021-03-24/text/original/epub/OEBPS/document_1/document_1.html#_Toc66194995> ;
    dcat:landingPage "https://www.legislation.gov.au/F2021L00317/asmade/2021-03-24/text/original/epub/OEBPS/document_1/document_1.html#_Toc66194995"^^xsd:anyURI ;
    dcat:theme legcons:Item .

F2021L00317:24 a legcons:Item,
        owl:Class,
        dcat:Resource ;
    rdfs:label "Item - I24 2 9  Conditions of exemptionmatters to which Secretary must have regard"@en-AU ;
    dct:isPartOf F2021L00317:11 ;
    dct:isReferencedBy F2021L00317: ;
    rdfs:comment "2 9  Conditions of exemptionmatters to which Secretary must have regard - Abrievated Graph Key: I24"@en-AU ;
    skos:definition "2 9  Conditions of exemptionmatters to which Secretary must have regard"@en-AU ;
    skos:narrower F2021L00317:11 ;
    skos:prefLabel "Item I24"@en-AU ;
    dcat:accessURL <https://www.legislation.gov.au/F2021L00317/asmade/2021-03-24/text/original/epub/OEBPS/document_1/document_1.html#_Toc66194781> ;
    dcat:landingPage "https://www.legislation.gov.au/F2021L00317/asmade/2021-03-24/text/original/epub/OEBPS/document_1/document_1.html#_Toc66194781"^^xsd:anyURI ;
    dcat:theme legcons:Item .

F2021L00317:240 a legcons:Item,
        owl:Class,
        dcat:Resource ;
    rdfs:label "Item - I240 9 32  Decisions that may be made by operation of computer program"@en-AU ;
    dct:isPartOf F2021L00317:239 ;
    dct:isReferencedBy F2021L00317: ;
    rdfs:comment "9 32  Decisions that may be made by operation of computer program - Abrievated Graph Key: I240"@en-AU ;
    skos:definition "9 32  Decisions that may be made by operation of computer program"@en-AU ;
    skos:narrower F2021L00317:239 ;
    skos:prefLabel "Item I240"@en-AU ;
    dcat:accessURL <https://www.legislation.gov.au/F2021L00317/asmade/2021-03-24/text/original/epub/OEBPS/document_1/document_1.html#_Toc66194997> ;
    dcat:landingPage "https://www.legislation.gov.au/F2021L00317/asmade/2021-03-24/text/original/epub/OEBPS/document_1/document_1.html#_Toc66194997"^^xsd:anyURI ;
    dcat:theme legcons:Item .

F2021L00317:243 a legcons:Item,
        owl:Class,
        dcat:Resource ;
    rdfs:label "Item - I243 9 33  Requirement to be third party authorised officerfit and proper person etc"@en-AU ;
    dct:isPartOf F2021L00317:242 ;
    dct:isReferencedBy F2021L00317: ;
    rdfs:comment "9 33  Requirement to be third party authorised officerfit and proper person etc - Abrievated Graph Key: I243"@en-AU ;
    skos:definition "9 33  Requirement to be third party authorised officerfit and proper person etc"@en-AU ;
    skos:narrower F2021L00317:242 ;
    skos:prefLabel "Item I243"@en-AU ;
    dcat:accessURL <https://www.legislation.gov.au/F2021L00317/asmade/2021-03-24/text/original/epub/OEBPS/document_1/document_1.html#_Toc66195000> ;
    dcat:landingPage "https://www.legislation.gov.au/F2021L00317/asmade/2021-03-24/text/original/epub/OEBPS/document_1/document_1.html#_Toc66195000"^^xsd:anyURI ;
    dcat:theme legcons:Item .

F2021L00317:245 a legcons:Item,
        owl:Class,
        dcat:Resource ;
    rdfs:label "Item - I245 9 34  Purpose of this Division"@en-AU ;
    dct:isPartOf F2021L00317:244 ;
    dct:isReferencedBy F2021L00317: ;
    rdfs:comment "9 34  Purpose of this Division - Abrievated Graph Key: I245"@en-AU ;
    skos:definition "9 34  Purpose of this Division"@en-AU ;
    skos:narrower F2021L00317:244 ;
    skos:prefLabel "Item I245"@en-AU ;
    dcat:accessURL <https://www.legislation.gov.au/F2021L00317/asmade/2021-03-24/text/original/epub/OEBPS/document_1/document_1.html#_Toc66195002> ;
    dcat:landingPage "https://www.legislation.gov.au/F2021L00317/asmade/2021-03-24/text/original/epub/OEBPS/document_1/document_1.html#_Toc66195002"^^xsd:anyURI ;
    dcat:theme legcons:Item .

F2021L00317:246 a legcons:Item,
        owl:Class,
        dcat:Resource ;
    rdfs:label "Item - I246 9 35  Inspecting establishments and securing areas equipment facilities or other things"@en-AU ;
    dct:isPartOf F2021L00317:244 ;
    dct:isReferencedBy F2021L00317: ;
    rdfs:comment "9 35  Inspecting establishments and securing areas equipment facilities or other things - Abrievated Graph Key: I246"@en-AU ;
    skos:definition "9 35  Inspecting establishments and securing areas equipment facilities or other things"@en-AU ;
    skos:narrower F2021L00317:244 ;
    skos:prefLabel "Item I246"@en-AU ;
    dcat:accessURL <https://www.legislation.gov.au/F2021L00317/asmade/2021-03-24/text/original/epub/OEBPS/document_1/document_1.html#_Toc66195003> ;
    dcat:landingPage "https://www.legislation.gov.au/F2021L00317/asmade/2021-03-24/text/original/epub/OEBPS/document_1/document_1.html#_Toc66195003"^^xsd:anyURI ;
    dcat:theme legcons:Item .

F2021L00317:247 a legcons:Item,
        owl:Class,
        dcat:Resource ;
    rdfs:label "Item - I247 9 36  Securing and identifying establishment or conveyance etc"@en-AU ;
    dct:isPartOf F2021L00317:244 ;
    dct:isReferencedBy F2021L00317: ;
    rdfs:comment "9 36  Securing and identifying establishment or conveyance etc - Abrievated Graph Key: I247"@en-AU ;
    skos:definition "9 36  Securing and identifying establishment or conveyance etc"@en-AU ;
    skos:narrower F2021L00317:244 ;
    skos:prefLabel "Item I247"@en-AU ;
    dcat:accessURL <https://www.legislation.gov.au/F2021L00317/asmade/2021-03-24/text/original/epub/OEBPS/document_1/document_1.html#_Toc66195004> ;
    dcat:landingPage "https://www.legislation.gov.au/F2021L00317/asmade/2021-03-24/text/original/epub/OEBPS/document_1/document_1.html#_Toc66195004"^^xsd:anyURI ;
    dcat:theme legcons:Item .

F2021L00317:248 a legcons:Item,
        owl:Class,
        dcat:Resource ;
    rdfs:label "Item - I248 9 37  Interference with identified establishment or conveyance etc"@en-AU ;
    dct:isPartOf F2021L00317:244 ;
    dct:isReferencedBy F2021L00317: ;
    rdfs:comment "9 37  Interference with identified establishment or conveyance etc - Abrievated Graph Key: I248"@en-AU ;
    skos:definition "9 37  Interference with identified establishment or conveyance etc"@en-AU ;
    skos:narrower F2021L00317:244 ;
    skos:prefLabel "Item I248"@en-AU ;
    dcat:accessURL <https://www.legislation.gov.au/F2021L00317/asmade/2021-03-24/text/original/epub/OEBPS/document_1/document_1.html#_Toc66195005> ;
    dcat:landingPage "https://www.legislation.gov.au/F2021L00317/asmade/2021-03-24/text/original/epub/OEBPS/document_1/document_1.html#_Toc66195005"^^xsd:anyURI ;
    dcat:theme legcons:Item .

F2021L00317:25 a legcons:Item,
        owl:Class,
        dcat:Resource ;
    rdfs:label "Item - I25 2 10  Instrument of exemption"@en-AU ;
    dct:isPartOf F2021L00317:11 ;
    dct:isReferencedBy F2021L00317: ;
    rdfs:comment "2 10  Instrument of exemption - Abrievated Graph Key: I25"@en-AU ;
    skos:definition "2 10  Instrument of exemption"@en-AU ;
    skos:narrower F2021L00317:11 ;
    skos:prefLabel "Item I25"@en-AU ;
    dcat:accessURL <https://www.legislation.gov.au/F2021L00317/asmade/2021-03-24/text/original/epub/OEBPS/document_1/document_1.html#_Toc66194782> ;
    dcat:landingPage "https://www.legislation.gov.au/F2021L00317/asmade/2021-03-24/text/original/epub/OEBPS/document_1/document_1.html#_Toc66194782"^^xsd:anyURI ;
    dcat:theme legcons:Item .

F2021L00317:250 a legcons:Item,
        owl:Class,
        dcat:Resource ;
    rdfs:label "Item - I250 9 38  Other grounds for giving direction"@en-AU ;
    dct:isPartOf F2021L00317:249 ;
    dct:isReferencedBy F2021L00317: ;
    rdfs:comment "9 38  Other grounds for giving direction - Abrievated Graph Key: I250"@en-AU ;
    skos:definition "9 38  Other grounds for giving direction"@en-AU ;
    skos:narrower F2021L00317:249 ;
    skos:prefLabel "Item I250"@en-AU ;
    dcat:accessURL <https://www.legislation.gov.au/F2021L00317/asmade/2021-03-24/text/original/epub/OEBPS/document_1/document_1.html#_Toc66195007> ;
    dcat:landingPage "https://www.legislation.gov.au/F2021L00317/asmade/2021-03-24/text/original/epub/OEBPS/document_1/document_1.html#_Toc66195007"^^xsd:anyURI ;
    dcat:theme legcons:Item .

F2021L00317:252 a legcons:Item,
        owl:Class,
        dcat:Resource ;
    rdfs:label "Item - I252 9 39  Circumstances in which identity card need not be carried"@en-AU ;
    dct:isPartOf F2021L00317:251 ;
    dct:isReferencedBy F2021L00317: ;
    rdfs:comment "9 39  Circumstances in which identity card need not be carried - Abrievated Graph Key: I252"@en-AU ;
    skos:definition "9 39  Circumstances in which identity card need not be carried"@en-AU ;
    skos:narrower F2021L00317:251 ;
    skos:prefLabel "Item I252"@en-AU ;
    dcat:accessURL <https://www.legislation.gov.au/F2021L00317/asmade/2021-03-24/text/original/epub/OEBPS/document_1/document_1.html#_Toc66195009> ;
    dcat:landingPage "https://www.legislation.gov.au/F2021L00317/asmade/2021-03-24/text/original/epub/OEBPS/document_1/document_1.html#_Toc66195009"^^xsd:anyURI ;
    dcat:theme legcons:Item .

F2021L00317:254 a legcons:Item,
        owl:Class,
        dcat:Resource ;
    rdfs:label "Item - I254 10 1  Samples taken in exercising monitoring or investigation powers"@en-AU ;
    dct:isPartOf F2021L00317:253 ;
    dct:isReferencedBy F2021L00317: ;
    rdfs:comment "10 1  Samples taken in exercising monitoring or investigation powers - Abrievated Graph Key: I254"@en-AU ;
    skos:definition "10 1  Samples taken in exercising monitoring or investigation powers"@en-AU ;
    skos:narrower F2021L00317:253 ;
    skos:prefLabel "Item I254"@en-AU ;
    dcat:accessURL <https://www.legislation.gov.au/F2021L00317/asmade/2021-03-24/text/original/epub/OEBPS/document_1/document_1.html#_Toc66195011> ;
    dcat:landingPage "https://www.legislation.gov.au/F2021L00317/asmade/2021-03-24/text/original/epub/OEBPS/document_1/document_1.html#_Toc66195011"^^xsd:anyURI ;
    dcat:theme legcons:Item .

F2021L00317:255 a legcons:Item,
        owl:Class,
        dcat:Resource ;
    rdfs:label "Item - I255 10 2  Dealing with things seized in exercising investigation powers"@en-AU ;
    dct:isPartOf F2021L00317:253 ;
    dct:isReferencedBy F2021L00317: ;
    rdfs:comment "10 2  Dealing with things seized in exercising investigation powers - Abrievated Graph Key: I255"@en-AU ;
    skos:definition "10 2  Dealing with things seized in exercising investigation powers"@en-AU ;
    skos:narrower F2021L00317:253 ;
    skos:prefLabel "Item I255"@en-AU ;
    dcat:accessURL <https://www.legislation.gov.au/F2021L00317/asmade/2021-03-24/text/original/epub/OEBPS/document_1/document_1.html#_Toc66195012> ;
    dcat:landingPage "https://www.legislation.gov.au/F2021L00317/asmade/2021-03-24/text/original/epub/OEBPS/document_1/document_1.html#_Toc66195012"^^xsd:anyURI ;
    dcat:theme legcons:Item .

F2021L00317:258 a legcons:Item,
        owl:Class,
        dcat:Resource ;
    rdfs:label "Item - I258 11 1  Reviewable decisions"@en-AU ;
    dct:isPartOf F2021L00317:257 ;
    dct:isReferencedBy F2021L00317: ;
    rdfs:comment "11 1  Reviewable decisions - Abrievated Graph Key: I258"@en-AU ;
    skos:definition "11 1  Reviewable decisions"@en-AU ;
    skos:narrower F2021L00317:257 ;
    skos:prefLabel "Item I258"@en-AU ;
    dcat:accessURL <https://www.legislation.gov.au/F2021L00317/asmade/2021-03-24/text/original/epub/OEBPS/document_1/document_1.html#_Toc66195015> ;
    dcat:landingPage "https://www.legislation.gov.au/F2021L00317/asmade/2021-03-24/text/original/epub/OEBPS/document_1/document_1.html#_Toc66195015"^^xsd:anyURI ;
    dcat:theme legcons:Item .

F2021L00317:26 a legcons:Item,
        owl:Class,
        dcat:Resource ;
    rdfs:label "Item - I26 2 11  Period of effect of exemption"@en-AU ;
    dct:isPartOf F2021L00317:11 ;
    dct:isReferencedBy F2021L00317: ;
    rdfs:comment "2 11  Period of effect of exemption - Abrievated Graph Key: I26"@en-AU ;
    skos:definition "2 11  Period of effect of exemption"@en-AU ;
    skos:narrower F2021L00317:11 ;
    skos:prefLabel "Item I26"@en-AU ;
    dcat:accessURL <https://www.legislation.gov.au/F2021L00317/asmade/2021-03-24/text/original/epub/OEBPS/document_1/document_1.html#_Toc66194783> ;
    dcat:landingPage "https://www.legislation.gov.au/F2021L00317/asmade/2021-03-24/text/original/epub/OEBPS/document_1/document_1.html#_Toc66194783"^^xsd:anyURI ;
    dcat:theme legcons:Item .

F2021L00317:260 a legcons:Item,
        owl:Class,
        dcat:Resource ;
    rdfs:label "Item - I260 11 2  Purpose of this Part"@en-AU ;
    dct:isPartOf F2021L00317:259 ;
    dct:isReferencedBy F2021L00317: ;
    rdfs:comment "11 2  Purpose of this Part - Abrievated Graph Key: I260"@en-AU ;
    skos:definition "11 2  Purpose of this Part"@en-AU ;
    skos:narrower F2021L00317:259 ;
    skos:prefLabel "Item I260"@en-AU ;
    dcat:accessURL <https://www.legislation.gov.au/F2021L00317/asmade/2021-03-24/text/original/epub/OEBPS/document_1/document_1.html#_Toc66195017> ;
    dcat:landingPage "https://www.legislation.gov.au/F2021L00317/asmade/2021-03-24/text/original/epub/OEBPS/document_1/document_1.html#_Toc66195017"^^xsd:anyURI ;
    dcat:theme legcons:Item .

F2021L00317:261 a legcons:Item,
        owl:Class,
        dcat:Resource ;
    rdfs:label "Item - I261 11 3  General requirements for records"@en-AU ;
    dct:isPartOf F2021L00317:259 ;
    dct:isReferencedBy F2021L00317: ;
    rdfs:comment "11 3  General requirements for records - Abrievated Graph Key: I261"@en-AU ;
    skos:definition "11 3  General requirements for records"@en-AU ;
    skos:narrower F2021L00317:259 ;
    skos:prefLabel "Item I261"@en-AU ;
    dcat:accessURL <https://www.legislation.gov.au/F2021L00317/asmade/2021-03-24/text/original/epub/OEBPS/document_1/document_1.html#_Toc66195018> ;
    dcat:landingPage "https://www.legislation.gov.au/F2021L00317/asmade/2021-03-24/text/original/epub/OEBPS/document_1/document_1.html#_Toc66195018"^^xsd:anyURI ;
    dcat:theme legcons:Item .

F2021L00317:262 a legcons:Item,
        owl:Class,
        dcat:Resource ;
    rdfs:label "Item - I262 11 4  Government certificates"@en-AU ;
    dct:isPartOf F2021L00317:259 ;
    dct:isReferencedBy F2021L00317: ;
    rdfs:comment "11 4  Government certificates - Abrievated Graph Key: I262"@en-AU ;
    skos:definition "11 4  Government certificates"@en-AU ;
    skos:narrower F2021L00317:259 ;
    skos:prefLabel "Item I262"@en-AU ;
    dcat:accessURL <https://www.legislation.gov.au/F2021L00317/asmade/2021-03-24/text/original/epub/OEBPS/document_1/document_1.html#_Toc66195019> ;
    dcat:landingPage "https://www.legislation.gov.au/F2021L00317/asmade/2021-03-24/text/original/epub/OEBPS/document_1/document_1.html#_Toc66195019"^^xsd:anyURI ;
    dcat:theme legcons:Item .

F2021L00317:263 a legcons:Item,
        owl:Class,
        dcat:Resource ;
    rdfs:label "Item - I263 11 5  Export permits"@en-AU ;
    dct:isPartOf F2021L00317:259 ;
    dct:isReferencedBy F2021L00317: ;
    rdfs:comment "11 5  Export permits - Abrievated Graph Key: I263"@en-AU ;
    skos:definition "11 5  Export permits"@en-AU ;
    skos:narrower F2021L00317:259 ;
    skos:prefLabel "Item I263"@en-AU ;
    dcat:accessURL <https://www.legislation.gov.au/F2021L00317/asmade/2021-03-24/text/original/epub/OEBPS/document_1/document_1.html#_Toc66195020> ;
    dcat:landingPage "https://www.legislation.gov.au/F2021L00317/asmade/2021-03-24/text/original/epub/OEBPS/document_1/document_1.html#_Toc66195020"^^xsd:anyURI ;
    dcat:theme legcons:Item .

F2021L00317:264 a legcons:Item,
        owl:Class,
        dcat:Resource ;
    rdfs:label "Item - I264 11 6  Records to be retained by exporter"@en-AU ;
    dct:isPartOf F2021L00317:259 ;
    dct:isReferencedBy F2021L00317: ;
    rdfs:comment "11 6  Records to be retained by exporter - Abrievated Graph Key: I264"@en-AU ;
    skos:definition "11 6  Records to be retained by exporter"@en-AU ;
    skos:narrower F2021L00317:259 ;
    skos:prefLabel "Item I264"@en-AU ;
    dcat:accessURL <https://www.legislation.gov.au/F2021L00317/asmade/2021-03-24/text/original/epub/OEBPS/document_1/document_1.html#_Toc66195021> ;
    dcat:landingPage "https://www.legislation.gov.au/F2021L00317/asmade/2021-03-24/text/original/epub/OEBPS/document_1/document_1.html#_Toc66195021"^^xsd:anyURI ;
    dcat:theme legcons:Item .

F2021L00317:265 a legcons:Item,
        owl:Class,
        dcat:Resource ;
    rdfs:label "Item - I265 11 7  Records to be retained by occupier of registered establishment"@en-AU ;
    dct:isPartOf F2021L00317:259 ;
    dct:isReferencedBy F2021L00317: ;
    rdfs:comment "11 7  Records to be retained by occupier of registered establishment - Abrievated Graph Key: I265"@en-AU ;
    skos:definition "11 7  Records to be retained by occupier of registered establishment"@en-AU ;
    skos:narrower F2021L00317:259 ;
    skos:prefLabel "Item I265"@en-AU ;
    dcat:accessURL <https://www.legislation.gov.au/F2021L00317/asmade/2021-03-24/text/original/epub/OEBPS/document_1/document_1.html#_Toc66195022> ;
    dcat:landingPage "https://www.legislation.gov.au/F2021L00317/asmade/2021-03-24/text/original/epub/OEBPS/document_1/document_1.html#_Toc66195022"^^xsd:anyURI ;
    dcat:theme legcons:Item .

F2021L00317:266 a legcons:Item,
        owl:Class,
        dcat:Resource ;
    rdfs:label "Item - I266 11 8  Records to be retained by holder of approved arrangement"@en-AU ;
    dct:isPartOf F2021L00317:259 ;
    dct:isReferencedBy F2021L00317: ;
    rdfs:comment "11 8  Records to be retained by holder of approved arrangement - Abrievated Graph Key: I266"@en-AU ;
    skos:definition "11 8  Records to be retained by holder of approved arrangement"@en-AU ;
    skos:narrower F2021L00317:259 ;
    skos:prefLabel "Item I266"@en-AU ;
    dcat:accessURL <https://www.legislation.gov.au/F2021L00317/asmade/2021-03-24/text/original/epub/OEBPS/document_1/document_1.html#_Toc66195023> ;
    dcat:landingPage "https://www.legislation.gov.au/F2021L00317/asmade/2021-03-24/text/original/epub/OEBPS/document_1/document_1.html#_Toc66195023"^^xsd:anyURI ;
    dcat:theme legcons:Item .

F2021L00317:267 a legcons:Item,
        owl:Class,
        dcat:Resource ;
    rdfs:label "Item - I267 11 9  Records relating to official marking devices"@en-AU ;
    dct:isPartOf F2021L00317:259 ;
    dct:isReferencedBy F2021L00317: ;
    rdfs:comment "11 9  Records relating to official marking devices - Abrievated Graph Key: I267"@en-AU ;
    skos:definition "11 9  Records relating to official marking devices"@en-AU ;
    skos:narrower F2021L00317:259 ;
    skos:prefLabel "Item I267"@en-AU ;
    dcat:accessURL <https://www.legislation.gov.au/F2021L00317/asmade/2021-03-24/text/original/epub/OEBPS/document_1/document_1.html#_Toc66195024> ;
    dcat:landingPage "https://www.legislation.gov.au/F2021L00317/asmade/2021-03-24/text/original/epub/OEBPS/document_1/document_1.html#_Toc66195024"^^xsd:anyURI ;
    dcat:theme legcons:Item .

F2021L00317:268 a legcons:Item,
        owl:Class,
        dcat:Resource ;
    rdfs:label "Item - I268 11 10  Records must not be altered or defaced during retention period"@en-AU ;
    dct:isPartOf F2021L00317:259 ;
    dct:isReferencedBy F2021L00317: ;
    rdfs:comment "11 10  Records must not be altered or defaced during retention period - Abrievated Graph Key: I268"@en-AU ;
    skos:definition "11 10  Records must not be altered or defaced during retention period"@en-AU ;
    skos:narrower F2021L00317:259 ;
    skos:prefLabel "Item I268"@en-AU ;
    dcat:accessURL <https://www.legislation.gov.au/F2021L00317/asmade/2021-03-24/text/original/epub/OEBPS/document_1/document_1.html#_Toc66195025> ;
    dcat:landingPage "https://www.legislation.gov.au/F2021L00317/asmade/2021-03-24/text/original/epub/OEBPS/document_1/document_1.html#_Toc66195025"^^xsd:anyURI ;
    dcat:theme legcons:Item .

F2021L00317:27 a legcons:Item,
        owl:Class,
        dcat:Resource ;
    rdfs:label "Item - I27 2 12  Variation of conditions of exemptionmatters to which Secretary must have regard"@en-AU ;
    dct:isPartOf F2021L00317:11 ;
    dct:isReferencedBy F2021L00317: ;
    rdfs:comment "2 12  Variation of conditions of exemptionmatters to which Secretary must have regard - Abrievated Graph Key: I27"@en-AU ;
    skos:definition "2 12  Variation of conditions of exemptionmatters to which Secretary must have regard"@en-AU ;
    skos:narrower F2021L00317:11 ;
    skos:prefLabel "Item I27"@en-AU ;
    dcat:accessURL <https://www.legislation.gov.au/F2021L00317/asmade/2021-03-24/text/original/epub/OEBPS/document_1/document_1.html#_Toc66194784> ;
    dcat:landingPage "https://www.legislation.gov.au/F2021L00317/asmade/2021-03-24/text/original/epub/OEBPS/document_1/document_1.html#_Toc66194784"^^xsd:anyURI ;
    dcat:theme legcons:Item .

F2021L00317:270 a legcons:Item,
        owl:Class,
        dcat:Resource ;
    rdfs:label "Item - I270 11 11  Microbiological limitstaking testing and analysing samples"@en-AU ;
    dct:isPartOf F2021L00317:269 ;
    dct:isReferencedBy F2021L00317: ;
    rdfs:comment "11 11  Microbiological limitstaking testing and analysing samples - Abrievated Graph Key: I270"@en-AU ;
    skos:definition "11 11  Microbiological limitstaking testing and analysing samples"@en-AU ;
    skos:narrower F2021L00317:269 ;
    skos:prefLabel "Item I270"@en-AU ;
    dcat:accessURL <https://www.legislation.gov.au/F2021L00317/asmade/2021-03-24/text/original/epub/OEBPS/document_1/document_1.html#_Toc66195027> ;
    dcat:landingPage "https://www.legislation.gov.au/F2021L00317/asmade/2021-03-24/text/original/epub/OEBPS/document_1/document_1.html#_Toc66195027"^^xsd:anyURI ;
    dcat:theme legcons:Item .

F2021L00317:271 a legcons:Item,
        owl:Class,
        dcat:Resource ;
    rdfs:label "Item - I271 11 12  Storage of samples"@en-AU ;
    dct:isPartOf F2021L00317:269 ;
    dct:isReferencedBy F2021L00317: ;
    rdfs:comment "11 12  Storage of samples - Abrievated Graph Key: I271"@en-AU ;
    skos:definition "11 12  Storage of samples"@en-AU ;
    skos:narrower F2021L00317:269 ;
    skos:prefLabel "Item I271"@en-AU ;
    dcat:accessURL <https://www.legislation.gov.au/F2021L00317/asmade/2021-03-24/text/original/epub/OEBPS/document_1/document_1.html#_Toc66195028> ;
    dcat:landingPage "https://www.legislation.gov.au/F2021L00317/asmade/2021-03-24/text/original/epub/OEBPS/document_1/document_1.html#_Toc66195028"^^xsd:anyURI ;
    dcat:theme legcons:Item .

F2021L00317:273 a legcons:Item,
        owl:Class,
        dcat:Resource ;
    rdfs:label "Item - I273 11 13  Division of compensation between owners"@en-AU ;
    dct:isPartOf F2021L00317:272 ;
    dct:isReferencedBy F2021L00317: ;
    rdfs:comment "11 13  Division of compensation between owners - Abrievated Graph Key: I273"@en-AU ;
    skos:definition "11 13  Division of compensation between owners"@en-AU ;
    skos:narrower F2021L00317:272 ;
    skos:prefLabel "Item I273"@en-AU ;
    dcat:accessURL <https://www.legislation.gov.au/F2021L00317/asmade/2021-03-24/text/original/epub/OEBPS/document_1/document_1.html#_Toc66195030> ;
    dcat:landingPage "https://www.legislation.gov.au/F2021L00317/asmade/2021-03-24/text/original/epub/OEBPS/document_1/document_1.html#_Toc66195030"^^xsd:anyURI ;
    dcat:theme legcons:Item .

F2021L00317:274 a legcons:Item,
        owl:Class,
        dcat:Resource ;
    rdfs:label "Item - I274 11 14  Amount of compensation"@en-AU ;
    dct:isPartOf F2021L00317:272 ;
    dct:isReferencedBy F2021L00317: ;
    rdfs:comment "11 14  Amount of compensation - Abrievated Graph Key: I274"@en-AU ;
    skos:definition "11 14  Amount of compensation"@en-AU ;
    skos:narrower F2021L00317:272 ;
    skos:prefLabel "Item I274"@en-AU ;
    dcat:accessURL <https://www.legislation.gov.au/F2021L00317/asmade/2021-03-24/text/original/epub/OEBPS/document_1/document_1.html#_Toc66195031> ;
    dcat:landingPage "https://www.legislation.gov.au/F2021L00317/asmade/2021-03-24/text/original/epub/OEBPS/document_1/document_1.html#_Toc66195031"^^xsd:anyURI ;
    dcat:theme legcons:Item .

F2021L00317:276 a legcons:Item,
        owl:Class,
        dcat:Resource ;
    rdfs:label "Item - I276 11 15  Circumstances in which relevant Commonwealth liability of a person is taken to have been paid"@en-AU ;
    dct:isPartOf F2021L00317:275 ;
    dct:isReferencedBy F2021L00317: ;
    rdfs:comment "11 15  Circumstances in which relevant Commonwealth liability of a person is taken to have been paid - Abrievated Graph Key: I276"@en-AU ;
    skos:definition "11 15  Circumstances in which relevant Commonwealth liability of a person is taken to have been paid"@en-AU ;
    skos:narrower F2021L00317:275 ;
    skos:prefLabel "Item I276"@en-AU ;
    dcat:accessURL <https://www.legislation.gov.au/F2021L00317/asmade/2021-03-24/text/original/epub/OEBPS/document_1/document_1.html#_Toc66195033> ;
    dcat:landingPage "https://www.legislation.gov.au/F2021L00317/asmade/2021-03-24/text/original/epub/OEBPS/document_1/document_1.html#_Toc66195033"^^xsd:anyURI ;
    dcat:theme legcons:Item .

F2021L00317:279 a legcons:Item,
        owl:Class,
        dcat:Resource ;
    rdfs:label "Item - I279 12 1  Definitions"@en-AU ;
    dct:isPartOf F2021L00317:278 ;
    dct:isReferencedBy F2021L00317: ;
    rdfs:comment "12 1  Definitions - Abrievated Graph Key: I279"@en-AU ;
    skos:definition "12 1  Definitions"@en-AU ;
    skos:narrower F2021L00317:278 ;
    skos:prefLabel "Item I279"@en-AU ;
    dcat:accessURL <https://www.legislation.gov.au/F2021L00317/asmade/2021-03-24/text/original/epub/OEBPS/document_1/document_1.html#_Toc66195036> ;
    dcat:landingPage "https://www.legislation.gov.au/F2021L00317/asmade/2021-03-24/text/original/epub/OEBPS/document_1/document_1.html#_Toc66195036"^^xsd:anyURI ;
    dcat:theme legcons:Item .

F2021L00317:28 a legcons:Part,
        owl:Class,
        dcat:Resource ;
    rdfs:label "Part - P28 Part 3 Government certificates"@en-AU ;
    dct:isPartOf F2021L00317:11 ;
    dct:isReferencedBy F2021L00317: ;
    rdfs:comment "Part 3 Government certificates - Abrievated Graph Key: P28"@en-AU ;
    skos:definition "Part 3 Government certificates"@en-AU ;
    skos:narrower F2021L00317:11 ;
    skos:prefLabel "Part P28"@en-AU ;
    dcat:accessURL <https://www.legislation.gov.au/F2021L00317/asmade/2021-03-24/text/original/epub/OEBPS/document_1/document_1.html#_Toc66194785> ;
    dcat:landingPage "https://www.legislation.gov.au/F2021L00317/asmade/2021-03-24/text/original/epub/OEBPS/document_1/document_1.html#_Toc66194785"^^xsd:anyURI ;
    dcat:theme legcons:Part .

F2021L00317:281 a legcons:Item,
        owl:Class,
        dcat:Resource ;
    rdfs:label "Item - I281 12 2  Information and declarations given before commencement time"@en-AU ;
    dct:isPartOf F2021L00317:280 ;
    dct:isReferencedBy F2021L00317: ;
    rdfs:comment "12 2  Information and declarations given before commencement time - Abrievated Graph Key: I281"@en-AU ;
    skos:definition "12 2  Information and declarations given before commencement time"@en-AU ;
    skos:narrower F2021L00317:280 ;
    skos:prefLabel "Item I281"@en-AU ;
    dcat:accessURL <https://www.legislation.gov.au/F2021L00317/asmade/2021-03-24/text/original/epub/OEBPS/document_1/document_1.html#_Toc66195038> ;
    dcat:landingPage "https://www.legislation.gov.au/F2021L00317/asmade/2021-03-24/text/original/epub/OEBPS/document_1/document_1.html#_Toc66195038"^^xsd:anyURI ;
    dcat:theme legcons:Item .

F2021L00317:284 a legcons:Item,
        owl:Class,
        dcat:Resource ;
    rdfs:label "Item - I284 12 3  Request for translation not complied with before commencement time"@en-AU ;
    dct:isPartOf F2021L00317:283 ;
    dct:isReferencedBy F2021L00317: ;
    rdfs:comment "12 3  Request for translation not complied with before commencement time - Abrievated Graph Key: I284"@en-AU ;
    skos:definition "12 3  Request for translation not complied with before commencement time"@en-AU ;
    skos:narrower F2021L00317:283 ;
    skos:prefLabel "Item I284"@en-AU ;
    dcat:accessURL <https://www.legislation.gov.au/F2021L00317/asmade/2021-03-24/text/original/epub/OEBPS/document_1/document_1.html#_Toc66195041> ;
    dcat:landingPage "https://www.legislation.gov.au/F2021L00317/asmade/2021-03-24/text/original/epub/OEBPS/document_1/document_1.html#_Toc66195041"^^xsd:anyURI ;
    dcat:theme legcons:Item .

F2021L00317:286 a legcons:Item,
        owl:Class,
        dcat:Resource ;
    rdfs:label "Item - I286 12 4  Person approved before commencement time to manufacture an official mark"@en-AU ;
    dct:isPartOf F2021L00317:285 ;
    dct:isReferencedBy F2021L00317: ;
    rdfs:comment "12 4  Person approved before commencement time to manufacture an official mark - Abrievated Graph Key: I286"@en-AU ;
    skos:definition "12 4  Person approved before commencement time to manufacture an official mark"@en-AU ;
    skos:narrower F2021L00317:285 ;
    skos:prefLabel "Item I286"@en-AU ;
    dcat:accessURL <https://www.legislation.gov.au/F2021L00317/asmade/2021-03-24/text/original/epub/OEBPS/document_1/document_1.html#_Toc66195043> ;
    dcat:landingPage "https://www.legislation.gov.au/F2021L00317/asmade/2021-03-24/text/original/epub/OEBPS/document_1/document_1.html#_Toc66195043"^^xsd:anyURI ;
    dcat:theme legcons:Item .

F2021L00317:287 a legcons:Item,
        owl:Class,
        dcat:Resource ;
    rdfs:label "Item - I287 12 5  Person approved before commencement time to possess an official mark"@en-AU ;
    dct:isPartOf F2021L00317:285 ;
    dct:isReferencedBy F2021L00317: ;
    rdfs:comment "12 5  Person approved before commencement time to possess an official mark - Abrievated Graph Key: I287"@en-AU ;
    skos:definition "12 5  Person approved before commencement time to possess an official mark"@en-AU ;
    skos:narrower F2021L00317:285 ;
    skos:prefLabel "Item I287"@en-AU ;
    dcat:accessURL <https://www.legislation.gov.au/F2021L00317/asmade/2021-03-24/text/original/epub/OEBPS/document_1/document_1.html#_Toc66195044> ;
    dcat:landingPage "https://www.legislation.gov.au/F2021L00317/asmade/2021-03-24/text/original/epub/OEBPS/document_1/document_1.html#_Toc66195044"^^xsd:anyURI ;
    dcat:theme legcons:Item .

F2021L00317:288 a legcons:Item,
        owl:Class,
        dcat:Resource ;
    rdfs:label "Item - I288 12 6  Person approved before commencement time to apply an official mark"@en-AU ;
    dct:isPartOf F2021L00317:285 ;
    dct:isReferencedBy F2021L00317: ;
    rdfs:comment "12 6  Person approved before commencement time to apply an official mark - Abrievated Graph Key: I288"@en-AU ;
    skos:definition "12 6  Person approved before commencement time to apply an official mark"@en-AU ;
    skos:narrower F2021L00317:285 ;
    skos:prefLabel "Item I288"@en-AU ;
    dcat:accessURL <https://www.legislation.gov.au/F2021L00317/asmade/2021-03-24/text/original/epub/OEBPS/document_1/document_1.html#_Toc66195045> ;
    dcat:landingPage "https://www.legislation.gov.au/F2021L00317/asmade/2021-03-24/text/original/epub/OEBPS/document_1/document_1.html#_Toc66195045"^^xsd:anyURI ;
    dcat:theme legcons:Item .

F2021L00317:29 a legcons:Item,
        owl:Class,
        dcat:Resource ;
    rdfs:label "Item - I29 2 13  When government certificate may be issued in relation to fish or fish products"@en-AU ;
    dct:isPartOf F2021L00317:11 ;
    dct:isReferencedBy F2021L00317: ;
    rdfs:comment "2 13  When government certificate may be issued in relation to fish or fish products - Abrievated Graph Key: I29"@en-AU ;
    skos:definition "2 13  When government certificate may be issued in relation to fish or fish products"@en-AU ;
    skos:narrower F2021L00317:11 ;
    skos:prefLabel "Item I29"@en-AU ;
    dcat:accessURL <https://www.legislation.gov.au/F2021L00317/asmade/2021-03-24/text/original/epub/OEBPS/document_1/document_1.html#_Toc66194786> ;
    dcat:landingPage "https://www.legislation.gov.au/F2021L00317/asmade/2021-03-24/text/original/epub/OEBPS/document_1/document_1.html#_Toc66194786"^^xsd:anyURI ;
    dcat:theme legcons:Item .

F2021L00317:290 a legcons:Item,
        owl:Class,
        dcat:Resource ;
    rdfs:label "Item - I290 12 7  Person approved before commencement time to manufacture an official marking device"@en-AU ;
    dct:isPartOf F2021L00317:289 ;
    dct:isReferencedBy F2021L00317: ;
    rdfs:comment "12 7  Person approved before commencement time to manufacture an official marking device - Abrievated Graph Key: I290"@en-AU ;
    skos:definition "12 7  Person approved before commencement time to manufacture an official marking device"@en-AU ;
    skos:narrower F2021L00317:289 ;
    skos:prefLabel "Item I290"@en-AU ;
    dcat:accessURL <https://www.legislation.gov.au/F2021L00317/asmade/2021-03-24/text/original/epub/OEBPS/document_1/document_1.html#_Toc66195047> ;
    dcat:landingPage "https://www.legislation.gov.au/F2021L00317/asmade/2021-03-24/text/original/epub/OEBPS/document_1/document_1.html#_Toc66195047"^^xsd:anyURI ;
    dcat:theme legcons:Item .

F2021L00317:291 a legcons:Item,
        owl:Class,
        dcat:Resource ;
    rdfs:label "Item - I291 12 8  Person approved before commencement time to possess an official marking device"@en-AU ;
    dct:isPartOf F2021L00317:289 ;
    dct:isReferencedBy F2021L00317: ;
    rdfs:comment "12 8  Person approved before commencement time to possess an official marking device - Abrievated Graph Key: I291"@en-AU ;
    skos:definition "12 8  Person approved before commencement time to possess an official marking device"@en-AU ;
    skos:narrower F2021L00317:289 ;
    skos:prefLabel "Item I291"@en-AU ;
    dcat:accessURL <https://www.legislation.gov.au/F2021L00317/asmade/2021-03-24/text/original/epub/OEBPS/document_1/document_1.html#_Toc66195048> ;
    dcat:landingPage "https://www.legislation.gov.au/F2021L00317/asmade/2021-03-24/text/original/epub/OEBPS/document_1/document_1.html#_Toc66195048"^^xsd:anyURI ;
    dcat:theme legcons:Item .

F2021L00317:294 a legcons:Item,
        owl:Class,
        dcat:Resource ;
    rdfs:label "Item - I294 12 9  Application for approval as auditor not decided or notice of decision not given before commencement time"@en-AU ;
    dct:isPartOf F2021L00317:293 ;
    dct:isReferencedBy F2021L00317: ;
    rdfs:comment "12 9  Application for approval as auditor not decided or notice of decision not given before commencement time - Abrievated Graph Key: I294"@en-AU ;
    skos:definition "12 9  Application for approval as auditor not decided or notice of decision not given before commencement time"@en-AU ;
    skos:narrower F2021L00317:293 ;
    skos:prefLabel "Item I294"@en-AU ;
    dcat:accessURL <https://www.legislation.gov.au/F2021L00317/asmade/2021-03-24/text/original/epub/OEBPS/document_1/document_1.html#_Toc66195051> ;
    dcat:landingPage "https://www.legislation.gov.au/F2021L00317/asmade/2021-03-24/text/original/epub/OEBPS/document_1/document_1.html#_Toc66195051"^^xsd:anyURI ;
    dcat:theme legcons:Item .

F2021L00317:295 a legcons:Item,
        owl:Class,
        dcat:Resource ;
    rdfs:label "Item - I295 12 10  Request for further information not complied with before commencement time"@en-AU ;
    dct:isPartOf F2021L00317:293 ;
    dct:isReferencedBy F2021L00317: ;
    rdfs:comment "12 10  Request for further information not complied with before commencement time - Abrievated Graph Key: I295"@en-AU ;
    skos:definition "12 10  Request for further information not complied with before commencement time"@en-AU ;
    skos:narrower F2021L00317:293 ;
    skos:prefLabel "Item I295"@en-AU ;
    dcat:accessURL <https://www.legislation.gov.au/F2021L00317/asmade/2021-03-24/text/original/epub/OEBPS/document_1/document_1.html#_Toc66195052> ;
    dcat:landingPage "https://www.legislation.gov.au/F2021L00317/asmade/2021-03-24/text/original/epub/OEBPS/document_1/document_1.html#_Toc66195052"^^xsd:anyURI ;
    dcat:theme legcons:Item .

F2021L00317:296 a legcons:Item,
        owl:Class,
        dcat:Resource ;
    rdfs:label "Item - I296 12 11  Decision to revoke approval as auditor decided but notice not given before commencement time"@en-AU ;
    dct:isPartOf F2021L00317:293 ;
    dct:isReferencedBy F2021L00317: ;
    rdfs:comment "12 11  Decision to revoke approval as auditor decided but notice not given before commencement time - Abrievated Graph Key: I296"@en-AU ;
    skos:definition "12 11  Decision to revoke approval as auditor decided but notice not given before commencement time"@en-AU ;
    skos:narrower F2021L00317:293 ;
    skos:prefLabel "Item I296"@en-AU ;
    dcat:accessURL <https://www.legislation.gov.au/F2021L00317/asmade/2021-03-24/text/original/epub/OEBPS/document_1/document_1.html#_Toc66195053> ;
    dcat:landingPage "https://www.legislation.gov.au/F2021L00317/asmade/2021-03-24/text/original/epub/OEBPS/document_1/document_1.html#_Toc66195053"^^xsd:anyURI ;
    dcat:theme legcons:Item .

F2021L00317:298 a legcons:Item,
        owl:Class,
        dcat:Resource ;
    rdfs:label "Item - I298 12 12  Verification by authorised officer before commencement time"@en-AU ;
    dct:isPartOf F2021L00317:297 ;
    dct:isReferencedBy F2021L00317: ;
    rdfs:comment "12 12  Verification by authorised officer before commencement time - Abrievated Graph Key: I298"@en-AU ;
    skos:definition "12 12  Verification by authorised officer before commencement time"@en-AU ;
    skos:narrower F2021L00317:297 ;
    skos:prefLabel "Item I298"@en-AU ;
    dcat:accessURL <https://www.legislation.gov.au/F2021L00317/asmade/2021-03-24/text/original/epub/OEBPS/document_1/document_1.html#_Toc66195055> ;
    dcat:landingPage "https://www.legislation.gov.au/F2021L00317/asmade/2021-03-24/text/original/epub/OEBPS/document_1/document_1.html#_Toc66195055"^^xsd:anyURI ;
    dcat:theme legcons:Item .

F2021L00317:3 a legcons:Item,
        owl:Class,
        dcat:Resource ;
    rdfs:label "Item - I3 1 1  Name"@en-AU ;
    dct:isPartOf F2021L00317:1 ;
    dct:isReferencedBy F2021L00317: ;
    rdfs:comment "1 1  Name - Abrievated Graph Key: I3"@en-AU ;
    skos:definition "1 1  Name"@en-AU ;
    skos:narrower F2021L00317:1 ;
    skos:prefLabel "Item I3"@en-AU ;
    dcat:accessURL <https://www.legislation.gov.au/F2021L00317/asmade/2021-03-24/text/original/epub/OEBPS/document_1/document_1.html#_Toc66194760> ;
    dcat:landingPage "https://www.legislation.gov.au/F2021L00317/asmade/2021-03-24/text/original/epub/OEBPS/document_1/document_1.html#_Toc66194760"^^xsd:anyURI ;
    dcat:theme legcons:Item .

F2021L00317:30 a legcons:Item,
        owl:Class,
        dcat:Resource ;
    rdfs:label "Item - I30 2 14  Matters stated in government certificatemanufacturing grade fish or fish products"@en-AU ;
    dct:isPartOf F2021L00317:11 ;
    dct:isReferencedBy F2021L00317: ;
    rdfs:comment "2 14  Matters stated in government certificatemanufacturing grade fish or fish products - Abrievated Graph Key: I30"@en-AU ;
    skos:definition "2 14  Matters stated in government certificatemanufacturing grade fish or fish products"@en-AU ;
    skos:narrower F2021L00317:11 ;
    skos:prefLabel "Item I30"@en-AU ;
    dcat:accessURL <https://www.legislation.gov.au/F2021L00317/asmade/2021-03-24/text/original/epub/OEBPS/document_1/document_1.html#_Toc66194787> ;
    dcat:landingPage "https://www.legislation.gov.au/F2021L00317/asmade/2021-03-24/text/original/epub/OEBPS/document_1/document_1.html#_Toc66194787"^^xsd:anyURI ;
    dcat:theme legcons:Item .

F2021L00317:31 a legcons:Item,
        owl:Class,
        dcat:Resource ;
    rdfs:label "Item - I31 2 15  Requirements before issue of government certificatecondition of fish or fish products"@en-AU ;
    dct:isPartOf F2021L00317:11 ;
    dct:isReferencedBy F2021L00317: ;
    rdfs:comment "2 15  Requirements before issue of government certificatecondition of fish or fish products - Abrievated Graph Key: I31"@en-AU ;
    skos:definition "2 15  Requirements before issue of government certificatecondition of fish or fish products"@en-AU ;
    skos:narrower F2021L00317:11 ;
    skos:prefLabel "Item I31"@en-AU ;
    dcat:accessURL <https://www.legislation.gov.au/F2021L00317/asmade/2021-03-24/text/original/epub/OEBPS/document_1/document_1.html#_Toc66194788> ;
    dcat:landingPage "https://www.legislation.gov.au/F2021L00317/asmade/2021-03-24/text/original/epub/OEBPS/document_1/document_1.html#_Toc66194788"^^xsd:anyURI ;
    dcat:theme legcons:Item .

F2021L00317:32 a legcons:Item,
        owl:Class,
        dcat:Resource ;
    rdfs:label "Item - I32 2 16  Circumstances for refusing to issue government certificate"@en-AU ;
    dct:isPartOf F2021L00317:11 ;
    dct:isReferencedBy F2021L00317: ;
    rdfs:comment "2 16  Circumstances for refusing to issue government certificate - Abrievated Graph Key: I32"@en-AU ;
    skos:definition "2 16  Circumstances for refusing to issue government certificate"@en-AU ;
    skos:narrower F2021L00317:11 ;
    skos:prefLabel "Item I32"@en-AU ;
    dcat:accessURL <https://www.legislation.gov.au/F2021L00317/asmade/2021-03-24/text/original/epub/OEBPS/document_1/document_1.html#_Toc66194789> ;
    dcat:landingPage "https://www.legislation.gov.au/F2021L00317/asmade/2021-03-24/text/original/epub/OEBPS/document_1/document_1.html#_Toc66194789"^^xsd:anyURI ;
    dcat:theme legcons:Item .

F2021L00317:33 a legcons:Item,
        owl:Class,
        dcat:Resource ;
    rdfs:label "Item - I33 2 17  Changes that require holder of certificate to give additional or corrected information to issuing body"@en-AU ;
    dct:isPartOf F2021L00317:11 ;
    dct:isReferencedBy F2021L00317: ;
    rdfs:comment "2 17  Changes that require holder of certificate to give additional or corrected information to issuing body - Abrievated Graph Key: I33"@en-AU ;
    skos:definition "2 17  Changes that require holder of certificate to give additional or corrected information to issuing body"@en-AU ;
    skos:narrower F2021L00317:11 ;
    skos:prefLabel "Item I33"@en-AU ;
    dcat:accessURL <https://www.legislation.gov.au/F2021L00317/asmade/2021-03-24/text/original/epub/OEBPS/document_1/document_1.html#_Toc66194790> ;
    dcat:landingPage "https://www.legislation.gov.au/F2021L00317/asmade/2021-03-24/text/original/epub/OEBPS/document_1/document_1.html#_Toc66194790"^^xsd:anyURI ;
    dcat:theme legcons:Item .

F2021L00317:34 a legcons:Item,
        owl:Class,
        dcat:Resource ;
    rdfs:label "Item - I34 2 18  Return of government certificate"@en-AU ;
    dct:isPartOf F2021L00317:11 ;
    dct:isReferencedBy F2021L00317: ;
    rdfs:comment "2 18  Return of government certificate - Abrievated Graph Key: I34"@en-AU ;
    skos:definition "2 18  Return of government certificate"@en-AU ;
    skos:narrower F2021L00317:11 ;
    skos:prefLabel "Item I34"@en-AU ;
    dcat:accessURL <https://www.legislation.gov.au/F2021L00317/asmade/2021-03-24/text/original/epub/OEBPS/document_1/document_1.html#_Toc66194791> ;
    dcat:landingPage "https://www.legislation.gov.au/F2021L00317/asmade/2021-03-24/text/original/epub/OEBPS/document_1/document_1.html#_Toc66194791"^^xsd:anyURI ;
    dcat:theme legcons:Item .

F2021L00317:38 a legcons:Item,
        owl:Class,
        dcat:Resource ;
    rdfs:label "Item - I38 4 1  Purpose of this Division"@en-AU ;
    dct:isPartOf F2021L00317:37 ;
    dct:isReferencedBy F2021L00317: ;
    rdfs:comment "4 1  Purpose of this Division - Abrievated Graph Key: I38"@en-AU ;
    skos:definition "4 1  Purpose of this Division"@en-AU ;
    skos:narrower F2021L00317:37 ;
    skos:prefLabel "Item I38"@en-AU ;
    dcat:accessURL <https://www.legislation.gov.au/F2021L00317/asmade/2021-03-24/text/original/epub/OEBPS/document_1/document_1.html#_Toc66194795> ;
    dcat:landingPage "https://www.legislation.gov.au/F2021L00317/asmade/2021-03-24/text/original/epub/OEBPS/document_1/document_1.html#_Toc66194795"^^xsd:anyURI ;
    dcat:theme legcons:Item .

F2021L00317:39 a legcons:Item,
        owl:Class,
        dcat:Resource ;
    rdfs:label "Item - I39 4 2  Equipment facilities and essential servicesgeneral"@en-AU ;
    dct:isPartOf F2021L00317:37 ;
    dct:isReferencedBy F2021L00317: ;
    rdfs:comment "4 2  Equipment facilities and essential servicesgeneral - Abrievated Graph Key: I39"@en-AU ;
    skos:definition "4 2  Equipment facilities and essential servicesgeneral"@en-AU ;
    skos:narrower F2021L00317:37 ;
    skos:prefLabel "Item I39"@en-AU ;
    dcat:accessURL <https://www.legislation.gov.au/F2021L00317/asmade/2021-03-24/text/original/epub/OEBPS/document_1/document_1.html#_Toc66194796> ;
    dcat:landingPage "https://www.legislation.gov.au/F2021L00317/asmade/2021-03-24/text/original/epub/OEBPS/document_1/document_1.html#_Toc66194796"^^xsd:anyURI ;
    dcat:theme legcons:Item .

F2021L00317:4 a legcons:Item,
        owl:Class,
        dcat:Resource ;
    rdfs:label "Item - I4 1 2  Commencement"@en-AU ;
    dct:isPartOf F2021L00317:1 ;
    dct:isReferencedBy F2021L00317: ;
    rdfs:comment "1 2  Commencement - Abrievated Graph Key: I4"@en-AU ;
    skos:definition "1 2  Commencement"@en-AU ;
    skos:narrower F2021L00317:1 ;
    skos:prefLabel "Item I4"@en-AU ;
    dcat:accessURL <https://www.legislation.gov.au/F2021L00317/asmade/2021-03-24/text/original/epub/OEBPS/document_1/document_1.html#_Toc66194761> ;
    dcat:landingPage "https://www.legislation.gov.au/F2021L00317/asmade/2021-03-24/text/original/epub/OEBPS/document_1/document_1.html#_Toc66194761"^^xsd:anyURI ;
    dcat:theme legcons:Item .

F2021L00317:40 a legcons:Item,
        owl:Class,
        dcat:Resource ;
    rdfs:label "Item - I40 4 3  Measuring devices"@en-AU ;
    dct:isPartOf F2021L00317:37 ;
    dct:isReferencedBy F2021L00317: ;
    rdfs:comment "4 3  Measuring devices - Abrievated Graph Key: I40"@en-AU ;
    skos:definition "4 3  Measuring devices"@en-AU ;
    skos:narrower F2021L00317:37 ;
    skos:prefLabel "Item I40"@en-AU ;
    dcat:accessURL <https://www.legislation.gov.au/F2021L00317/asmade/2021-03-24/text/original/epub/OEBPS/document_1/document_1.html#_Toc66194797> ;
    dcat:landingPage "https://www.legislation.gov.au/F2021L00317/asmade/2021-03-24/text/original/epub/OEBPS/document_1/document_1.html#_Toc66194797"^^xsd:anyURI ;
    dcat:theme legcons:Item .

F2021L00317:41 a legcons:Item,
        owl:Class,
        dcat:Resource ;
    rdfs:label "Item - I41 4 4  Establishment including construction"@en-AU ;
    dct:isPartOf F2021L00317:37 ;
    dct:isReferencedBy F2021L00317: ;
    rdfs:comment "4 4  Establishment including construction - Abrievated Graph Key: I41"@en-AU ;
    skos:definition "4 4  Establishment including construction"@en-AU ;
    skos:narrower F2021L00317:37 ;
    skos:prefLabel "Item I41"@en-AU ;
    dcat:accessURL <https://www.legislation.gov.au/F2021L00317/asmade/2021-03-24/text/original/epub/OEBPS/document_1/document_1.html#_Toc66194798> ;
    dcat:landingPage "https://www.legislation.gov.au/F2021L00317/asmade/2021-03-24/text/original/epub/OEBPS/document_1/document_1.html#_Toc66194798"^^xsd:anyURI ;
    dcat:theme legcons:Item .

F2021L00317:42 a legcons:Item,
        owl:Class,
        dcat:Resource ;
    rdfs:label "Item - I42 4 5  Fixtures fittings and equipment"@en-AU ;
    dct:isPartOf F2021L00317:37 ;
    dct:isReferencedBy F2021L00317: ;
    rdfs:comment "4 5  Fixtures fittings and equipment - Abrievated Graph Key: I42"@en-AU ;
    skos:definition "4 5  Fixtures fittings and equipment"@en-AU ;
    skos:narrower F2021L00317:37 ;
    skos:prefLabel "Item I42"@en-AU ;
    dcat:accessURL <https://www.legislation.gov.au/F2021L00317/asmade/2021-03-24/text/original/epub/OEBPS/document_1/document_1.html#_Toc66194799> ;
    dcat:landingPage "https://www.legislation.gov.au/F2021L00317/asmade/2021-03-24/text/original/epub/OEBPS/document_1/document_1.html#_Toc66194799"^^xsd:anyURI ;
    dcat:theme legcons:Item .

F2021L00317:43 a legcons:Item,
        owl:Class,
        dcat:Resource ;
    rdfs:label "Item - I43 4 6  Storage facilities for items other than fish or fish products"@en-AU ;
    dct:isPartOf F2021L00317:37 ;
    dct:isReferencedBy F2021L00317: ;
    rdfs:comment "4 6  Storage facilities for items other than fish or fish products - Abrievated Graph Key: I43"@en-AU ;
    skos:definition "4 6  Storage facilities for items other than fish or fish products"@en-AU ;
    skos:narrower F2021L00317:37 ;
    skos:prefLabel "Item I43"@en-AU ;
    dcat:accessURL <https://www.legislation.gov.au/F2021L00317/asmade/2021-03-24/text/original/epub/OEBPS/document_1/document_1.html#_Toc66194800> ;
    dcat:landingPage "https://www.legislation.gov.au/F2021L00317/asmade/2021-03-24/text/original/epub/OEBPS/document_1/document_1.html#_Toc66194800"^^xsd:anyURI ;
    dcat:theme legcons:Item .

F2021L00317:44 a legcons:Item,
        owl:Class,
        dcat:Resource ;
    rdfs:label "Item - I44 4 7  Cleaning and sanitising facilities"@en-AU ;
    dct:isPartOf F2021L00317:37 ;
    dct:isReferencedBy F2021L00317: ;
    rdfs:comment "4 7  Cleaning and sanitising facilities - Abrievated Graph Key: I44"@en-AU ;
    skos:definition "4 7  Cleaning and sanitising facilities"@en-AU ;
    skos:narrower F2021L00317:37 ;
    skos:prefLabel "Item I44"@en-AU ;
    dcat:accessURL <https://www.legislation.gov.au/F2021L00317/asmade/2021-03-24/text/original/epub/OEBPS/document_1/document_1.html#_Toc66194801> ;
    dcat:landingPage "https://www.legislation.gov.au/F2021L00317/asmade/2021-03-24/text/original/epub/OEBPS/document_1/document_1.html#_Toc66194801"^^xsd:anyURI ;
    dcat:theme legcons:Item .

F2021L00317:45 a legcons:Item,
        owl:Class,
        dcat:Resource ;
    rdfs:label "Item - I45 4 8  Amenities"@en-AU ;
    dct:isPartOf F2021L00317:37 ;
    dct:isReferencedBy F2021L00317: ;
    rdfs:comment "4 8  Amenities - Abrievated Graph Key: I45"@en-AU ;
    skos:definition "4 8  Amenities"@en-AU ;
    skos:narrower F2021L00317:37 ;
    skos:prefLabel "Item I45"@en-AU ;
    dcat:accessURL <https://www.legislation.gov.au/F2021L00317/asmade/2021-03-24/text/original/epub/OEBPS/document_1/document_1.html#_Toc66194802> ;
    dcat:landingPage "https://www.legislation.gov.au/F2021L00317/asmade/2021-03-24/text/original/epub/OEBPS/document_1/document_1.html#_Toc66194802"^^xsd:anyURI ;
    dcat:theme legcons:Item .

F2021L00317:46 a legcons:Item,
        owl:Class,
        dcat:Resource ;
    rdfs:label "Item - I46 4 9  Essential services"@en-AU ;
    dct:isPartOf F2021L00317:37 ;
    dct:isReferencedBy F2021L00317: ;
    rdfs:comment "4 9  Essential services - Abrievated Graph Key: I46"@en-AU ;
    skos:definition "4 9  Essential services"@en-AU ;
    skos:narrower F2021L00317:37 ;
    skos:prefLabel "Item I46"@en-AU ;
    dcat:accessURL <https://www.legislation.gov.au/F2021L00317/asmade/2021-03-24/text/original/epub/OEBPS/document_1/document_1.html#_Toc66194803> ;
    dcat:landingPage "https://www.legislation.gov.au/F2021L00317/asmade/2021-03-24/text/original/epub/OEBPS/document_1/document_1.html#_Toc66194803"^^xsd:anyURI ;
    dcat:theme legcons:Item .

F2021L00317:47 a legcons:Item,
        owl:Class,
        dcat:Resource ;
    rdfs:label "Item - I47 4 10  Fishing vessels etc"@en-AU ;
    dct:isPartOf F2021L00317:37 ;
    dct:isReferencedBy F2021L00317: ;
    rdfs:comment "4 10  Fishing vessels etc - Abrievated Graph Key: I47"@en-AU ;
    skos:definition "4 10  Fishing vessels etc"@en-AU ;
    skos:narrower F2021L00317:37 ;
    skos:prefLabel "Item I47"@en-AU ;
    dcat:accessURL <https://www.legislation.gov.au/F2021L00317/asmade/2021-03-24/text/original/epub/OEBPS/document_1/document_1.html#_Toc66194804> ;
    dcat:landingPage "https://www.legislation.gov.au/F2021L00317/asmade/2021-03-24/text/original/epub/OEBPS/document_1/document_1.html#_Toc66194804"^^xsd:anyURI ;
    dcat:theme legcons:Item .

F2021L00317:49 a legcons:Item,
        owl:Class,
        dcat:Resource ;
    rdfs:label "Item - I49 4 11  Purpose of this Division"@en-AU ;
    dct:isPartOf F2021L00317:48 ;
    dct:isReferencedBy F2021L00317: ;
    rdfs:comment "4 11  Purpose of this Division - Abrievated Graph Key: I49"@en-AU ;
    skos:definition "4 11  Purpose of this Division"@en-AU ;
    skos:narrower F2021L00317:48 ;
    skos:prefLabel "Item I49"@en-AU ;
    dcat:accessURL <https://www.legislation.gov.au/F2021L00317/asmade/2021-03-24/text/original/epub/OEBPS/document_1/document_1.html#_Toc66194806> ;
    dcat:landingPage "https://www.legislation.gov.au/F2021L00317/asmade/2021-03-24/text/original/epub/OEBPS/document_1/document_1.html#_Toc66194806"^^xsd:anyURI ;
    dcat:theme legcons:Item .

F2021L00317:5 a legcons:Item,
        owl:Class,
        dcat:Resource ;
    rdfs:label "Item - I5 1 3  Authority"@en-AU ;
    dct:isPartOf F2021L00317:1 ;
    dct:isReferencedBy F2021L00317: ;
    rdfs:comment "1 3  Authority - Abrievated Graph Key: I5"@en-AU ;
    skos:definition "1 3  Authority"@en-AU ;
    skos:narrower F2021L00317:1 ;
    skos:prefLabel "Item I5"@en-AU ;
    dcat:accessURL <https://www.legislation.gov.au/F2021L00317/asmade/2021-03-24/text/original/epub/OEBPS/document_1/document_1.html#_Toc66194762> ;
    dcat:landingPage "https://www.legislation.gov.au/F2021L00317/asmade/2021-03-24/text/original/epub/OEBPS/document_1/document_1.html#_Toc66194762"^^xsd:anyURI ;
    dcat:theme legcons:Item .

F2021L00317:50 a legcons:Item,
        owl:Class,
        dcat:Resource ;
    rdfs:label "Item - I50 4 12  Operations must be carried out in a way that will ensure requirements of the Act are met"@en-AU ;
    dct:isPartOf F2021L00317:48 ;
    dct:isReferencedBy F2021L00317: ;
    rdfs:comment "4 12  Operations must be carried out in a way that will ensure requirements of the Act are met - Abrievated Graph Key: I50"@en-AU ;
    skos:definition "4 12  Operations must be carried out in a way that will ensure requirements of the Act are met"@en-AU ;
    skos:narrower F2021L00317:48 ;
    skos:prefLabel "Item I50"@en-AU ;
    dcat:accessURL <https://www.legislation.gov.au/F2021L00317/asmade/2021-03-24/text/original/epub/OEBPS/document_1/document_1.html#_Toc66194807> ;
    dcat:landingPage "https://www.legislation.gov.au/F2021L00317/asmade/2021-03-24/text/original/epub/OEBPS/document_1/document_1.html#_Toc66194807"^^xsd:anyURI ;
    dcat:theme legcons:Item .

F2021L00317:52 a legcons:Item,
        owl:Class,
        dcat:Resource ;
    rdfs:label "Item - I52 4 13  Purpose of this Part"@en-AU ;
    dct:isPartOf F2021L00317:51 ;
    dct:isReferencedBy F2021L00317: ;
    rdfs:comment "4 13  Purpose of this Part - Abrievated Graph Key: I52"@en-AU ;
    skos:definition "4 13  Purpose of this Part"@en-AU ;
    skos:narrower F2021L00317:51 ;
    skos:prefLabel "Item I52"@en-AU ;
    dcat:accessURL <https://www.legislation.gov.au/F2021L00317/asmade/2021-03-24/text/original/epub/OEBPS/document_1/document_1.html#_Toc66194809> ;
    dcat:landingPage "https://www.legislation.gov.au/F2021L00317/asmade/2021-03-24/text/original/epub/OEBPS/document_1/document_1.html#_Toc66194809"^^xsd:anyURI ;
    dcat:theme legcons:Item .

F2021L00317:53 a legcons:Item,
        owl:Class,
        dcat:Resource ;
    rdfs:label "Item - I53 4 14  Requirements for registration continue to be met"@en-AU ;
    dct:isPartOf F2021L00317:51 ;
    dct:isReferencedBy F2021L00317: ;
    rdfs:comment "4 14  Requirements for registration continue to be met - Abrievated Graph Key: I53"@en-AU ;
    skos:definition "4 14  Requirements for registration continue to be met"@en-AU ;
    skos:narrower F2021L00317:51 ;
    skos:prefLabel "Item I53"@en-AU ;
    dcat:accessURL <https://www.legislation.gov.au/F2021L00317/asmade/2021-03-24/text/original/epub/OEBPS/document_1/document_1.html#_Toc66194810> ;
    dcat:landingPage "https://www.legislation.gov.au/F2021L00317/asmade/2021-03-24/text/original/epub/OEBPS/document_1/document_1.html#_Toc66194810"^^xsd:anyURI ;
    dcat:theme legcons:Item .

F2021L00317:54 a legcons:Item,
        owl:Class,
        dcat:Resource ;
    rdfs:label "Item - I54 4 15  Other operational hygiene requirements"@en-AU ;
    dct:isPartOf F2021L00317:51 ;
    dct:isReferencedBy F2021L00317: ;
    rdfs:comment "4 15  Other operational hygiene requirements - Abrievated Graph Key: I54"@en-AU ;
    skos:definition "4 15  Other operational hygiene requirements"@en-AU ;
    skos:narrower F2021L00317:51 ;
    skos:prefLabel "Item I54"@en-AU ;
    dcat:accessURL <https://www.legislation.gov.au/F2021L00317/asmade/2021-03-24/text/original/epub/OEBPS/document_1/document_1.html#_Toc66194811> ;
    dcat:landingPage "https://www.legislation.gov.au/F2021L00317/asmade/2021-03-24/text/original/epub/OEBPS/document_1/document_1.html#_Toc66194811"^^xsd:anyURI ;
    dcat:theme legcons:Item .

F2021L00317:56 a legcons:Item,
        owl:Class,
        dcat:Resource ;
    rdfs:label "Item - I56 4 16  Period within which application to renew registration must be made"@en-AU ;
    dct:isPartOf F2021L00317:55 ;
    dct:isReferencedBy F2021L00317: ;
    rdfs:comment "4 16  Period within which application to renew registration must be made - Abrievated Graph Key: I56"@en-AU ;
    skos:definition "4 16  Period within which application to renew registration must be made"@en-AU ;
    skos:narrower F2021L00317:55 ;
    skos:prefLabel "Item I56"@en-AU ;
    dcat:accessURL <https://www.legislation.gov.au/F2021L00317/asmade/2021-03-24/text/original/epub/OEBPS/document_1/document_1.html#_Toc66194813> ;
    dcat:landingPage "https://www.legislation.gov.au/F2021L00317/asmade/2021-03-24/text/original/epub/OEBPS/document_1/document_1.html#_Toc66194813"^^xsd:anyURI ;
    dcat:theme legcons:Item .

F2021L00317:57 a legcons:Item,
        owl:Class,
        dcat:Resource ;
    rdfs:label "Item - I57 4 17  Requirements for renewal of registration"@en-AU ;
    dct:isPartOf F2021L00317:55 ;
    dct:isReferencedBy F2021L00317: ;
    rdfs:comment "4 17  Requirements for renewal of registration - Abrievated Graph Key: I57"@en-AU ;
    skos:definition "4 17  Requirements for renewal of registration"@en-AU ;
    skos:narrower F2021L00317:55 ;
    skos:prefLabel "Item I57"@en-AU ;
    dcat:accessURL <https://www.legislation.gov.au/F2021L00317/asmade/2021-03-24/text/original/epub/OEBPS/document_1/document_1.html#_Toc66194814> ;
    dcat:landingPage "https://www.legislation.gov.au/F2021L00317/asmade/2021-03-24/text/original/epub/OEBPS/document_1/document_1.html#_Toc66194814"^^xsd:anyURI ;
    dcat:theme legcons:Item .

F2021L00317:59 a legcons:Item,
        owl:Class,
        dcat:Resource ;
    rdfs:label "Item - I59 4 18  Request by occupier for suspension"@en-AU ;
    dct:isPartOf F2021L00317:58 ;
    dct:isReferencedBy F2021L00317: ;
    rdfs:comment "4 18  Request by occupier for suspension - Abrievated Graph Key: I59"@en-AU ;
    skos:definition "4 18  Request by occupier for suspension"@en-AU ;
    skos:narrower F2021L00317:58 ;
    skos:prefLabel "Item I59"@en-AU ;
    dcat:accessURL <https://www.legislation.gov.au/F2021L00317/asmade/2021-03-24/text/original/epub/OEBPS/document_1/document_1.html#_Toc66194816> ;
    dcat:landingPage "https://www.legislation.gov.au/F2021L00317/asmade/2021-03-24/text/original/epub/OEBPS/document_1/document_1.html#_Toc66194816"^^xsd:anyURI ;
    dcat:theme legcons:Item .

F2021L00317:6 a legcons:Item,
        owl:Class,
        dcat:Resource ;
    rdfs:label "Item - I6 1 4  Extension of Act to Heard Island and McDonald Islands"@en-AU ;
    dct:isPartOf F2021L00317:1 ;
    dct:isReferencedBy F2021L00317: ;
    rdfs:comment "1 4  Extension of Act to Heard Island and McDonald Islands - Abrievated Graph Key: I6"@en-AU ;
    skos:definition "1 4  Extension of Act to Heard Island and McDonald Islands"@en-AU ;
    skos:narrower F2021L00317:1 ;
    skos:prefLabel "Item I6"@en-AU ;
    dcat:accessURL <https://www.legislation.gov.au/F2021L00317/asmade/2021-03-24/text/original/epub/OEBPS/document_1/document_1.html#_Toc66194763> ;
    dcat:landingPage "https://www.legislation.gov.au/F2021L00317/asmade/2021-03-24/text/original/epub/OEBPS/document_1/document_1.html#_Toc66194763"^^xsd:anyURI ;
    dcat:theme legcons:Item .

F2021L00317:60 a legcons:Item,
        owl:Class,
        dcat:Resource ;
    rdfs:label "Item - I60 4 19  Other grounds for suspension"@en-AU ;
    dct:isPartOf F2021L00317:58 ;
    dct:isReferencedBy F2021L00317: ;
    rdfs:comment "4 19  Other grounds for suspension - Abrievated Graph Key: I60"@en-AU ;
    skos:definition "4 19  Other grounds for suspension"@en-AU ;
    skos:narrower F2021L00317:58 ;
    skos:prefLabel "Item I60"@en-AU ;
    dcat:accessURL <https://www.legislation.gov.au/F2021L00317/asmade/2021-03-24/text/original/epub/OEBPS/document_1/document_1.html#_Toc66194817> ;
    dcat:landingPage "https://www.legislation.gov.au/F2021L00317/asmade/2021-03-24/text/original/epub/OEBPS/document_1/document_1.html#_Toc66194817"^^xsd:anyURI ;
    dcat:theme legcons:Item .

F2021L00317:62 a legcons:Item,
        owl:Class,
        dcat:Resource ;
    rdfs:label "Item - I62 4 20  Application of this Part"@en-AU ;
    dct:isPartOf F2021L00317:61 ;
    dct:isReferencedBy F2021L00317: ;
    rdfs:comment "4 20  Application of this Part - Abrievated Graph Key: I62"@en-AU ;
    skos:definition "4 20  Application of this Part"@en-AU ;
    skos:narrower F2021L00317:61 ;
    skos:prefLabel "Item I62"@en-AU ;
    dcat:accessURL <https://www.legislation.gov.au/F2021L00317/asmade/2021-03-24/text/original/epub/OEBPS/document_1/document_1.html#_Toc66194819> ;
    dcat:landingPage "https://www.legislation.gov.au/F2021L00317/asmade/2021-03-24/text/original/epub/OEBPS/document_1/document_1.html#_Toc66194819"^^xsd:anyURI ;
    dcat:theme legcons:Item .

F2021L00317:63 a legcons:Item,
        owl:Class,
        dcat:Resource ;
    rdfs:label "Item - I63 4 21  Initial consideration period"@en-AU ;
    dct:isPartOf F2021L00317:61 ;
    dct:isReferencedBy F2021L00317: ;
    rdfs:comment "4 21  Initial consideration period - Abrievated Graph Key: I63"@en-AU ;
    skos:definition "4 21  Initial consideration period"@en-AU ;
    skos:narrower F2021L00317:61 ;
    skos:prefLabel "Item I63"@en-AU ;
    dcat:accessURL <https://www.legislation.gov.au/F2021L00317/asmade/2021-03-24/text/original/epub/OEBPS/document_1/document_1.html#_Toc66194820> ;
    dcat:landingPage "https://www.legislation.gov.au/F2021L00317/asmade/2021-03-24/text/original/epub/OEBPS/document_1/document_1.html#_Toc66194820"^^xsd:anyURI ;
    dcat:theme legcons:Item .

F2021L00317:64 a legcons:Item,
        owl:Class,
        dcat:Resource ;
    rdfs:label "Item - I64 4 22  Period within which request relating to application must be complied with"@en-AU ;
    dct:isPartOf F2021L00317:61 ;
    dct:isReferencedBy F2021L00317: ;
    rdfs:comment "4 22  Period within which request relating to application must be complied with - Abrievated Graph Key: I64"@en-AU ;
    skos:definition "4 22  Period within which request relating to application must be complied with"@en-AU ;
    skos:narrower F2021L00317:61 ;
    skos:prefLabel "Item I64"@en-AU ;
    dcat:accessURL <https://www.legislation.gov.au/F2021L00317/asmade/2021-03-24/text/original/epub/OEBPS/document_1/document_1.html#_Toc66194821> ;
    dcat:landingPage "https://www.legislation.gov.au/F2021L00317/asmade/2021-03-24/text/original/epub/OEBPS/document_1/document_1.html#_Toc66194821"^^xsd:anyURI ;
    dcat:theme legcons:Item .

F2021L00317:67 a legcons:Item,
        owl:Class,
        dcat:Resource ;
    rdfs:label "Item - I67 5 1  Purpose of this Part"@en-AU ;
    dct:isPartOf F2021L00317:66 ;
    dct:isReferencedBy F2021L00317: ;
    rdfs:comment "5 1  Purpose of this Part - Abrievated Graph Key: I67"@en-AU ;
    skos:definition "5 1  Purpose of this Part"@en-AU ;
    skos:narrower F2021L00317:66 ;
    skos:prefLabel "Item I67"@en-AU ;
    dcat:accessURL <https://www.legislation.gov.au/F2021L00317/asmade/2021-03-24/text/original/epub/OEBPS/document_1/document_1.html#_Toc66194824> ;
    dcat:landingPage "https://www.legislation.gov.au/F2021L00317/asmade/2021-03-24/text/original/epub/OEBPS/document_1/document_1.html#_Toc66194824"^^xsd:anyURI ;
    dcat:theme legcons:Item .

F2021L00317:68 a legcons:Item,
        owl:Class,
        dcat:Resource ;
    rdfs:label "Item - I68 5 2  Proposed arrangement for operations to prepare prescribed fish or fish products"@en-AU ;
    dct:isPartOf F2021L00317:66 ;
    dct:isReferencedBy F2021L00317: ;
    rdfs:comment "5 2  Proposed arrangement for operations to prepare prescribed fish or fish products - Abrievated Graph Key: I68"@en-AU ;
    skos:definition "5 2  Proposed arrangement for operations to prepare prescribed fish or fish products"@en-AU ;
    skos:narrower F2021L00317:66 ;
    skos:prefLabel "Item I68"@en-AU ;
    dcat:accessURL <https://www.legislation.gov.au/F2021L00317/asmade/2021-03-24/text/original/epub/OEBPS/document_1/document_1.html#_Toc66194825> ;
    dcat:landingPage "https://www.legislation.gov.au/F2021L00317/asmade/2021-03-24/text/original/epub/OEBPS/document_1/document_1.html#_Toc66194825"^^xsd:anyURI ;
    dcat:theme legcons:Item .

F2021L00317:69 a legcons:Item,
        owl:Class,
        dcat:Resource ;
    rdfs:label "Item - I69 5 3  Equipment"@en-AU ;
    dct:isPartOf F2021L00317:66 ;
    dct:isReferencedBy F2021L00317: ;
    rdfs:comment "5 3  Equipment - Abrievated Graph Key: I69"@en-AU ;
    skos:definition "5 3  Equipment"@en-AU ;
    skos:narrower F2021L00317:66 ;
    skos:prefLabel "Item I69"@en-AU ;
    dcat:accessURL <https://www.legislation.gov.au/F2021L00317/asmade/2021-03-24/text/original/epub/OEBPS/document_1/document_1.html#_Toc66194826> ;
    dcat:landingPage "https://www.legislation.gov.au/F2021L00317/asmade/2021-03-24/text/original/epub/OEBPS/document_1/document_1.html#_Toc66194826"^^xsd:anyURI ;
    dcat:theme legcons:Item .

F2021L00317:7 a legcons:Item,
        owl:Class,
        dcat:Resource ;
    rdfs:label "Item - I7 1 5  Simplified outline of this instrument"@en-AU ;
    dct:isPartOf F2021L00317:1 ;
    dct:isReferencedBy F2021L00317: ;
    rdfs:comment "1 5  Simplified outline of this instrument - Abrievated Graph Key: I7"@en-AU ;
    skos:definition "1 5  Simplified outline of this instrument"@en-AU ;
    skos:narrower F2021L00317:1 ;
    skos:prefLabel "Item I7"@en-AU ;
    dcat:accessURL <https://www.legislation.gov.au/F2021L00317/asmade/2021-03-24/text/original/epub/OEBPS/document_1/document_1.html#_Toc66194764> ;
    dcat:landingPage "https://www.legislation.gov.au/F2021L00317/asmade/2021-03-24/text/original/epub/OEBPS/document_1/document_1.html#_Toc66194764"^^xsd:anyURI ;
    dcat:theme legcons:Item .

F2021L00317:70 a legcons:Item,
        owl:Class,
        dcat:Resource ;
    rdfs:label "Item - I70 5 4  Operational hygiene"@en-AU ;
    dct:isPartOf F2021L00317:66 ;
    dct:isReferencedBy F2021L00317: ;
    rdfs:comment "5 4  Operational hygiene - Abrievated Graph Key: I70"@en-AU ;
    skos:definition "5 4  Operational hygiene"@en-AU ;
    skos:narrower F2021L00317:66 ;
    skos:prefLabel "Item I70"@en-AU ;
    dcat:accessURL <https://www.legislation.gov.au/F2021L00317/asmade/2021-03-24/text/original/epub/OEBPS/document_1/document_1.html#_Toc66194827> ;
    dcat:landingPage "https://www.legislation.gov.au/F2021L00317/asmade/2021-03-24/text/original/epub/OEBPS/document_1/document_1.html#_Toc66194827"^^xsd:anyURI ;
    dcat:theme legcons:Item .

F2021L00317:71 a legcons:Item,
        owl:Class,
        dcat:Resource ;
    rdfs:label "Item - I71 5 5  Identification traceability and integrity"@en-AU ;
    dct:isPartOf F2021L00317:66 ;
    dct:isReferencedBy F2021L00317: ;
    rdfs:comment "5 5  Identification traceability and integrity - Abrievated Graph Key: I71"@en-AU ;
    skos:definition "5 5  Identification traceability and integrity"@en-AU ;
    skos:narrower F2021L00317:66 ;
    skos:prefLabel "Item I71"@en-AU ;
    dcat:accessURL <https://www.legislation.gov.au/F2021L00317/asmade/2021-03-24/text/original/epub/OEBPS/document_1/document_1.html#_Toc66194828> ;
    dcat:landingPage "https://www.legislation.gov.au/F2021L00317/asmade/2021-03-24/text/original/epub/OEBPS/document_1/document_1.html#_Toc66194828"^^xsd:anyURI ;
    dcat:theme legcons:Item .

F2021L00317:74 a legcons:Item,
        owl:Class,
        dcat:Resource ;
    rdfs:label "Item - I74 5 6  Purpose of this Part"@en-AU ;
    dct:isPartOf F2021L00317:73 ;
    dct:isReferencedBy F2021L00317: ;
    rdfs:comment "5 6  Purpose of this Part - Abrievated Graph Key: I74"@en-AU ;
    skos:definition "5 6  Purpose of this Part"@en-AU ;
    skos:narrower F2021L00317:73 ;
    skos:prefLabel "Item I74"@en-AU ;
    dcat:accessURL <https://www.legislation.gov.au/F2021L00317/asmade/2021-03-24/text/original/epub/OEBPS/document_1/document_1.html#_Toc66194831> ;
    dcat:landingPage "https://www.legislation.gov.au/F2021L00317/asmade/2021-03-24/text/original/epub/OEBPS/document_1/document_1.html#_Toc66194831"^^xsd:anyURI ;
    dcat:theme legcons:Item .

F2021L00317:76 a legcons:Item,
        owl:Class,
        dcat:Resource ;
    rdfs:label "Item - I76 5 7  Importing country requirements must be met"@en-AU ;
    dct:isPartOf F2021L00317:75 ;
    dct:isReferencedBy F2021L00317: ;
    rdfs:comment "5 7  Importing country requirements must be met - Abrievated Graph Key: I76"@en-AU ;
    skos:definition "5 7  Importing country requirements must be met"@en-AU ;
    skos:narrower F2021L00317:75 ;
    skos:prefLabel "Item I76"@en-AU ;
    dcat:accessURL <https://www.legislation.gov.au/F2021L00317/asmade/2021-03-24/text/original/epub/OEBPS/document_1/document_1.html#_Toc66194833> ;
    dcat:landingPage "https://www.legislation.gov.au/F2021L00317/asmade/2021-03-24/text/original/epub/OEBPS/document_1/document_1.html#_Toc66194833"^^xsd:anyURI ;
    dcat:theme legcons:Item .

F2021L00317:78 a legcons:Item,
        owl:Class,
        dcat:Resource ;
    rdfs:label "Item - I78 5 8  Purpose of this Division"@en-AU ;
    dct:isPartOf F2021L00317:77 ;
    dct:isReferencedBy F2021L00317: ;
    rdfs:comment "5 8  Purpose of this Division - Abrievated Graph Key: I78"@en-AU ;
    skos:definition "5 8  Purpose of this Division"@en-AU ;
    skos:narrower F2021L00317:77 ;
    skos:prefLabel "Item I78"@en-AU ;
    dcat:accessURL <https://www.legislation.gov.au/F2021L00317/asmade/2021-03-24/text/original/epub/OEBPS/document_1/document_1.html#_Toc66194835> ;
    dcat:landingPage "https://www.legislation.gov.au/F2021L00317/asmade/2021-03-24/text/original/epub/OEBPS/document_1/document_1.html#_Toc66194835"^^xsd:anyURI ;
    dcat:theme legcons:Item .

F2021L00317:8 a legcons:Part,
        owl:Class,
        dcat:Resource ;
    rdfs:label "Part - P8 Part 2 Interpretation"@en-AU ;
    dct:isPartOf F2021L00317:1 ;
    dct:isReferencedBy F2021L00317: ;
    rdfs:comment "Part 2 Interpretation - Abrievated Graph Key: P8"@en-AU ;
    skos:definition "Part 2 Interpretation"@en-AU ;
    skos:narrower F2021L00317:1 ;
    skos:prefLabel "Part P8"@en-AU ;
    dcat:accessURL <https://www.legislation.gov.au/F2021L00317/asmade/2021-03-24/text/original/epub/OEBPS/document_1/document_1.html#_Toc66194765> ;
    dcat:landingPage "https://www.legislation.gov.au/F2021L00317/asmade/2021-03-24/text/original/epub/OEBPS/document_1/document_1.html#_Toc66194765"^^xsd:anyURI ;
    dcat:theme legcons:Part .

F2021L00317:80 a legcons:Item,
        owl:Class,
        dcat:Resource ;
    rdfs:label "Item - I80 5 9  Hygiene controlestablishment and its equipment"@en-AU ;
    dct:isPartOf F2021L00317:79 ;
    dct:isReferencedBy F2021L00317: ;
    rdfs:comment "5 9  Hygiene controlestablishment and its equipment - Abrievated Graph Key: I80"@en-AU ;
    skos:definition "5 9  Hygiene controlestablishment and its equipment"@en-AU ;
    skos:narrower F2021L00317:79 ;
    skos:prefLabel "Item I80"@en-AU ;
    dcat:accessURL <https://www.legislation.gov.au/F2021L00317/asmade/2021-03-24/text/original/epub/OEBPS/document_1/document_1.html#_Toc66194837> ;
    dcat:landingPage "https://www.legislation.gov.au/F2021L00317/asmade/2021-03-24/text/original/epub/OEBPS/document_1/document_1.html#_Toc66194837"^^xsd:anyURI ;
    dcat:theme legcons:Item .

F2021L00317:81 a legcons:Item,
        owl:Class,
        dcat:Resource ;
    rdfs:label "Item - I81 5 10  Measuring devices"@en-AU ;
    dct:isPartOf F2021L00317:79 ;
    dct:isReferencedBy F2021L00317: ;
    rdfs:comment "5 10  Measuring devices - Abrievated Graph Key: I81"@en-AU ;
    skos:definition "5 10  Measuring devices"@en-AU ;
    skos:narrower F2021L00317:79 ;
    skos:prefLabel "Item I81"@en-AU ;
    dcat:accessURL <https://www.legislation.gov.au/F2021L00317/asmade/2021-03-24/text/original/epub/OEBPS/document_1/document_1.html#_Toc66194838> ;
    dcat:landingPage "https://www.legislation.gov.au/F2021L00317/asmade/2021-03-24/text/original/epub/OEBPS/document_1/document_1.html#_Toc66194838"^^xsd:anyURI ;
    dcat:theme legcons:Item .

F2021L00317:82 a legcons:Item,
        owl:Class,
        dcat:Resource ;
    rdfs:label "Item - I82 5 11  Hygiene controlprocessing"@en-AU ;
    dct:isPartOf F2021L00317:79 ;
    dct:isReferencedBy F2021L00317: ;
    rdfs:comment "5 11  Hygiene controlprocessing - Abrievated Graph Key: I82"@en-AU ;
    skos:definition "5 11  Hygiene controlprocessing"@en-AU ;
    skos:narrower F2021L00317:79 ;
    skos:prefLabel "Item I82"@en-AU ;
    dcat:accessURL <https://www.legislation.gov.au/F2021L00317/asmade/2021-03-24/text/original/epub/OEBPS/document_1/document_1.html#_Toc66194839> ;
    dcat:landingPage "https://www.legislation.gov.au/F2021L00317/asmade/2021-03-24/text/original/epub/OEBPS/document_1/document_1.html#_Toc66194839"^^xsd:anyURI ;
    dcat:theme legcons:Item .

F2021L00317:83 a legcons:Item,
        owl:Class,
        dcat:Resource ;
    rdfs:label "Item - I83 5 12  Personal hygiene and health"@en-AU ;
    dct:isPartOf F2021L00317:79 ;
    dct:isReferencedBy F2021L00317: ;
    rdfs:comment "5 12  Personal hygiene and health - Abrievated Graph Key: I83"@en-AU ;
    skos:definition "5 12  Personal hygiene and health"@en-AU ;
    skos:narrower F2021L00317:79 ;
    skos:prefLabel "Item I83"@en-AU ;
    dcat:accessURL <https://www.legislation.gov.au/F2021L00317/asmade/2021-03-24/text/original/epub/OEBPS/document_1/document_1.html#_Toc66194840> ;
    dcat:landingPage "https://www.legislation.gov.au/F2021L00317/asmade/2021-03-24/text/original/epub/OEBPS/document_1/document_1.html#_Toc66194840"^^xsd:anyURI ;
    dcat:theme legcons:Item .

F2021L00317:84 a legcons:Subdivision,
        owl:Class,
        dcat:Resource ;
    rdfs:label "Subdivision - S84 Subdivision BCrocodiles and crocodile meat"@en-AU ;
    dct:isPartOf F2021L00317:77 ;
    dct:isReferencedBy F2021L00317: ;
    rdfs:comment "Subdivision BCrocodiles and crocodile meat - Abrievated Graph Key: S84"@en-AU ;
    skos:definition "Subdivision BCrocodiles and crocodile meat"@en-AU ;
    skos:narrower F2021L00317:77 ;
    skos:prefLabel "Subdivision S84"@en-AU ;
    dcat:accessURL <https://www.legislation.gov.au/F2021L00317/asmade/2021-03-24/text/original/epub/OEBPS/document_1/document_1.html#_Toc66194841> ;
    dcat:landingPage "https://www.legislation.gov.au/F2021L00317/asmade/2021-03-24/text/original/epub/OEBPS/document_1/document_1.html#_Toc66194841"^^xsd:anyURI ;
    dcat:theme legcons:Subdivision .

F2021L00317:85 a legcons:Item,
        owl:Class,
        dcat:Resource ;
    rdfs:label "Item - I85 5 13  Hygiene controlequipment"@en-AU ;
    dct:isPartOf F2021L00317:77 ;
    dct:isReferencedBy F2021L00317: ;
    rdfs:comment "5 13  Hygiene controlequipment - Abrievated Graph Key: I85"@en-AU ;
    skos:definition "5 13  Hygiene controlequipment"@en-AU ;
    skos:narrower F2021L00317:77 ;
    skos:prefLabel "Item I85"@en-AU ;
    dcat:accessURL <https://www.legislation.gov.au/F2021L00317/asmade/2021-03-24/text/original/epub/OEBPS/document_1/document_1.html#_Toc66194842> ;
    dcat:landingPage "https://www.legislation.gov.au/F2021L00317/asmade/2021-03-24/text/original/epub/OEBPS/document_1/document_1.html#_Toc66194842"^^xsd:anyURI ;
    dcat:theme legcons:Item .

F2021L00317:86 a legcons:Item,
        owl:Class,
        dcat:Resource ;
    rdfs:label "Item - I86 5 14  Personal hygiene"@en-AU ;
    dct:isPartOf F2021L00317:77 ;
    dct:isReferencedBy F2021L00317: ;
    rdfs:comment "5 14  Personal hygiene - Abrievated Graph Key: I86"@en-AU ;
    skos:definition "5 14  Personal hygiene"@en-AU ;
    skos:narrower F2021L00317:77 ;
    skos:prefLabel "Item I86"@en-AU ;
    dcat:accessURL <https://www.legislation.gov.au/F2021L00317/asmade/2021-03-24/text/original/epub/OEBPS/document_1/document_1.html#_Toc66194843> ;
    dcat:landingPage "https://www.legislation.gov.au/F2021L00317/asmade/2021-03-24/text/original/epub/OEBPS/document_1/document_1.html#_Toc66194843"^^xsd:anyURI ;
    dcat:theme legcons:Item .

F2021L00317:87 a legcons:Division,
        owl:Class,
        dcat:Resource ;
    rdfs:label "Division - D87 Division 4 Preparation and transport"@en-AU ;
    dct:isPartOf F2021L00317:72 ;
    dct:isReferencedBy F2021L00317: ;
    rdfs:comment "Division 4 Preparation and transport - Abrievated Graph Key: D87"@en-AU ;
    skos:definition "Division 4 Preparation and transport"@en-AU ;
    skos:narrower F2021L00317:72 ;
    skos:prefLabel "Division D87"@en-AU ;
    dcat:accessURL <https://www.legislation.gov.au/F2021L00317/asmade/2021-03-24/text/original/epub/OEBPS/document_1/document_1.html#_Toc66194844> ;
    dcat:landingPage "https://www.legislation.gov.au/F2021L00317/asmade/2021-03-24/text/original/epub/OEBPS/document_1/document_1.html#_Toc66194844"^^xsd:anyURI ;
    dcat:theme legcons:Division .

F2021L00317:89 a legcons:Item,
        owl:Class,
        dcat:Resource ;
    rdfs:label "Item - I89 5 15  Fish or fish products not to be prepared for export as food"@en-AU ;
    dct:isPartOf F2021L00317:88 ;
    dct:isReferencedBy F2021L00317: ;
    rdfs:comment "5 15  Fish or fish products not to be prepared for export as food - Abrievated Graph Key: I89"@en-AU ;
    skos:definition "5 15  Fish or fish products not to be prepared for export as food"@en-AU ;
    skos:narrower F2021L00317:88 ;
    skos:prefLabel "Item I89"@en-AU ;
    dcat:accessURL <https://www.legislation.gov.au/F2021L00317/asmade/2021-03-24/text/original/epub/OEBPS/document_1/document_1.html#_Toc66194846> ;
    dcat:landingPage "https://www.legislation.gov.au/F2021L00317/asmade/2021-03-24/text/original/epub/OEBPS/document_1/document_1.html#_Toc66194846"^^xsd:anyURI ;
    dcat:theme legcons:Item .

F2021L00317:9 a legcons:Item,
        owl:Class,
        dcat:Resource ;
    rdfs:label "Item - I9 1 6  Definitions"@en-AU ;
    dct:isPartOf F2021L00317:1 ;
    dct:isReferencedBy F2021L00317: ;
    rdfs:comment "1 6  Definitions - Abrievated Graph Key: I9"@en-AU ;
    skos:definition "1 6  Definitions"@en-AU ;
    skos:narrower F2021L00317:1 ;
    skos:prefLabel "Item I9"@en-AU ;
    dcat:accessURL <https://www.legislation.gov.au/F2021L00317/asmade/2021-03-24/text/original/epub/OEBPS/document_1/document_1.html#_Toc66194766> ;
    dcat:landingPage "https://www.legislation.gov.au/F2021L00317/asmade/2021-03-24/text/original/epub/OEBPS/document_1/document_1.html#_Toc66194766"^^xsd:anyURI ;
    dcat:theme legcons:Item .

F2021L00317:90 a legcons:Item,
        owl:Class,
        dcat:Resource ;
    rdfs:label "Item - I90 5 16  Sourcing fish and fish products"@en-AU ;
    dct:isPartOf F2021L00317:88 ;
    dct:isReferencedBy F2021L00317: ;
    rdfs:comment "5 16  Sourcing fish and fish products - Abrievated Graph Key: I90"@en-AU ;
    skos:definition "5 16  Sourcing fish and fish products"@en-AU ;
    skos:narrower F2021L00317:88 ;
    skos:prefLabel "Item I90"@en-AU ;
    dcat:accessURL <https://www.legislation.gov.au/F2021L00317/asmade/2021-03-24/text/original/epub/OEBPS/document_1/document_1.html#_Toc66194847> ;
    dcat:landingPage "https://www.legislation.gov.au/F2021L00317/asmade/2021-03-24/text/original/epub/OEBPS/document_1/document_1.html#_Toc66194847"^^xsd:anyURI ;
    dcat:theme legcons:Item .

F2021L00317:91 a legcons:Item,
        owl:Class,
        dcat:Resource ;
    rdfs:label "Item - I91 5 17  Notifiable diseases"@en-AU ;
    dct:isPartOf F2021L00317:88 ;
    dct:isReferencedBy F2021L00317: ;
    rdfs:comment "5 17  Notifiable diseases - Abrievated Graph Key: I91"@en-AU ;
    skos:definition "5 17  Notifiable diseases"@en-AU ;
    skos:narrower F2021L00317:88 ;
    skos:prefLabel "Item I91"@en-AU ;
    dcat:accessURL <https://www.legislation.gov.au/F2021L00317/asmade/2021-03-24/text/original/epub/OEBPS/document_1/document_1.html#_Toc66194848> ;
    dcat:landingPage "https://www.legislation.gov.au/F2021L00317/asmade/2021-03-24/text/original/epub/OEBPS/document_1/document_1.html#_Toc66194848"^^xsd:anyURI ;
    dcat:theme legcons:Item .

F2021L00317:92 a legcons:Item,
        owl:Class,
        dcat:Resource ;
    rdfs:label "Item - I92 5 18  Temperature controls for preparing prescribed fish or fish products"@en-AU ;
    dct:isPartOf F2021L00317:88 ;
    dct:isReferencedBy F2021L00317: ;
    rdfs:comment "5 18  Temperature controls for preparing prescribed fish or fish products - Abrievated Graph Key: I92"@en-AU ;
    skos:definition "5 18  Temperature controls for preparing prescribed fish or fish products"@en-AU ;
    skos:narrower F2021L00317:88 ;
    skos:prefLabel "Item I92"@en-AU ;
    dcat:accessURL <https://www.legislation.gov.au/F2021L00317/asmade/2021-03-24/text/original/epub/OEBPS/document_1/document_1.html#_Toc66194849> ;
    dcat:landingPage "https://www.legislation.gov.au/F2021L00317/asmade/2021-03-24/text/original/epub/OEBPS/document_1/document_1.html#_Toc66194849"^^xsd:anyURI ;
    dcat:theme legcons:Item .

F2021L00317:93 a legcons:Item,
        owl:Class,
        dcat:Resource ;
    rdfs:label "Item - I93 5 19  Temperature controls for storing handling loading and transporting prescribed fish or fish products"@en-AU ;
    dct:isPartOf F2021L00317:88 ;
    dct:isReferencedBy F2021L00317: ;
    rdfs:comment "5 19  Temperature controls for storing handling loading and transporting prescribed fish or fish products - Abrievated Graph Key: I93"@en-AU ;
    skos:definition "5 19  Temperature controls for storing handling loading and transporting prescribed fish or fish products"@en-AU ;
    skos:narrower F2021L00317:88 ;
    skos:prefLabel "Item I93"@en-AU ;
    dcat:accessURL <https://www.legislation.gov.au/F2021L00317/asmade/2021-03-24/text/original/epub/OEBPS/document_1/document_1.html#_Toc66194850> ;
    dcat:landingPage "https://www.legislation.gov.au/F2021L00317/asmade/2021-03-24/text/original/epub/OEBPS/document_1/document_1.html#_Toc66194850"^^xsd:anyURI ;
    dcat:theme legcons:Item .

F2021L00317:94 a legcons:Item,
        owl:Class,
        dcat:Resource ;
    rdfs:label "Item - I94 5 20  Preserving prescribed fish and fish products"@en-AU ;
    dct:isPartOf F2021L00317:88 ;
    dct:isReferencedBy F2021L00317: ;
    rdfs:comment "5 20  Preserving prescribed fish and fish products - Abrievated Graph Key: I94"@en-AU ;
    skos:definition "5 20  Preserving prescribed fish and fish products"@en-AU ;
    skos:narrower F2021L00317:88 ;
    skos:prefLabel "Item I94"@en-AU ;
    dcat:accessURL <https://www.legislation.gov.au/F2021L00317/asmade/2021-03-24/text/original/epub/OEBPS/document_1/document_1.html#_Toc66194851> ;
    dcat:landingPage "https://www.legislation.gov.au/F2021L00317/asmade/2021-03-24/text/original/epub/OEBPS/document_1/document_1.html#_Toc66194851"^^xsd:anyURI ;
    dcat:theme legcons:Item .

F2021L00317:95 a legcons:Item,
        owl:Class,
        dcat:Resource ;
    rdfs:label "Item - I95 5 21  Thermal processing of canned prescribed fish or fish products"@en-AU ;
    dct:isPartOf F2021L00317:88 ;
    dct:isReferencedBy F2021L00317: ;
    rdfs:comment "5 21  Thermal processing of canned prescribed fish or fish products - Abrievated Graph Key: I95"@en-AU ;
    skos:definition "5 21  Thermal processing of canned prescribed fish or fish products"@en-AU ;
    skos:narrower F2021L00317:88 ;
    skos:prefLabel "Item I95"@en-AU ;
    dcat:accessURL <https://www.legislation.gov.au/F2021L00317/asmade/2021-03-24/text/original/epub/OEBPS/document_1/document_1.html#_Toc66194852> ;
    dcat:landingPage "https://www.legislation.gov.au/F2021L00317/asmade/2021-03-24/text/original/epub/OEBPS/document_1/document_1.html#_Toc66194852"^^xsd:anyURI ;
    dcat:theme legcons:Item .

F2021L00317:96 a legcons:Item,
        owl:Class,
        dcat:Resource ;
    rdfs:label "Item - I96 5 22  Packaging and identification"@en-AU ;
    dct:isPartOf F2021L00317:88 ;
    dct:isReferencedBy F2021L00317: ;
    rdfs:comment "5 22  Packaging and identification - Abrievated Graph Key: I96"@en-AU ;
    skos:definition "5 22  Packaging and identification"@en-AU ;
    skos:narrower F2021L00317:88 ;
    skos:prefLabel "Item I96"@en-AU ;
    dcat:accessURL <https://www.legislation.gov.au/F2021L00317/asmade/2021-03-24/text/original/epub/OEBPS/document_1/document_1.html#_Toc66194853> ;
    dcat:landingPage "https://www.legislation.gov.au/F2021L00317/asmade/2021-03-24/text/original/epub/OEBPS/document_1/document_1.html#_Toc66194853"^^xsd:anyURI ;
    dcat:theme legcons:Item .

F2021L00317:97 a legcons:Item,
        owl:Class,
        dcat:Resource ;
    rdfs:label "Item - I97 5 23  Storage handling and loading"@en-AU ;
    dct:isPartOf F2021L00317:88 ;
    dct:isReferencedBy F2021L00317: ;
    rdfs:comment "5 23  Storage handling and loading - Abrievated Graph Key: I97"@en-AU ;
    skos:definition "5 23  Storage handling and loading"@en-AU ;
    skos:narrower F2021L00317:88 ;
    skos:prefLabel "Item I97"@en-AU ;
    dcat:accessURL <https://www.legislation.gov.au/F2021L00317/asmade/2021-03-24/text/original/epub/OEBPS/document_1/document_1.html#_Toc66194854> ;
    dcat:landingPage "https://www.legislation.gov.au/F2021L00317/asmade/2021-03-24/text/original/epub/OEBPS/document_1/document_1.html#_Toc66194854"^^xsd:anyURI ;
    dcat:theme legcons:Item .

F2021L00317:98 a legcons:Item,
        owl:Class,
        dcat:Resource ;
    rdfs:label "Item - I98 5 24  Container system units and food carrying compartments of vehiclesconstruction etc"@en-AU ;
    dct:isPartOf F2021L00317:88 ;
    dct:isReferencedBy F2021L00317: ;
    rdfs:comment "5 24  Container system units and food carrying compartments of vehiclesconstruction etc - Abrievated Graph Key: I98"@en-AU ;
    skos:definition "5 24  Container system units and food carrying compartments of vehiclesconstruction etc"@en-AU ;
    skos:narrower F2021L00317:88 ;
    skos:prefLabel "Item I98"@en-AU ;
    dcat:accessURL <https://www.legislation.gov.au/F2021L00317/asmade/2021-03-24/text/original/epub/OEBPS/document_1/document_1.html#_Toc66194855> ;
    dcat:landingPage "https://www.legislation.gov.au/F2021L00317/asmade/2021-03-24/text/original/epub/OEBPS/document_1/document_1.html#_Toc66194855"^^xsd:anyURI ;
    dcat:theme legcons:Item .

F2021L00317:99 a legcons:Item,
        owl:Class,
        dcat:Resource ;
    rdfs:label "Item - I99 5 25  Vehicles container system units etchygiene control"@en-AU ;
    dct:isPartOf F2021L00317:88 ;
    dct:isReferencedBy F2021L00317: ;
    rdfs:comment "5 25  Vehicles container system units etchygiene control - Abrievated Graph Key: I99"@en-AU ;
    skos:definition "5 25  Vehicles container system units etchygiene control"@en-AU ;
    skos:narrower F2021L00317:88 ;
    skos:prefLabel "Item I99"@en-AU ;
    dcat:accessURL <https://www.legislation.gov.au/F2021L00317/asmade/2021-03-24/text/original/epub/OEBPS/document_1/document_1.html#_Toc66194856> ;
    dcat:landingPage "https://www.legislation.gov.au/F2021L00317/asmade/2021-03-24/text/original/epub/OEBPS/document_1/document_1.html#_Toc66194856"^^xsd:anyURI ;
    dcat:theme legcons:Item .

F2021L00317:138 a legcons:Division,
        owl:Class,
        dcat:Resource ;
    rdfs:label "Division - D138 Division 2 Variations required by Secretary"@en-AU ;
    dct:hasPart F2021L00317:139 ;
    dct:isPartOf F2021L00317:65 ;
    dct:isReferencedBy F2021L00317: ;
    rdfs:comment "Division 2 Variations required by Secretary - Abrievated Graph Key: D138"@en-AU ;
    skos:broader F2021L00317:139 ;
    skos:definition "Division 2 Variations required by Secretary"@en-AU ;
    skos:narrower F2021L00317:65 ;
    skos:prefLabel "Division D138"@en-AU ;
    dcat:accessURL <https://www.legislation.gov.au/F2021L00317/asmade/2021-03-24/text/original/epub/OEBPS/document_1/document_1.html#_Toc66194895> ;
    dcat:landingPage "https://www.legislation.gov.au/F2021L00317/asmade/2021-03-24/text/original/epub/OEBPS/document_1/document_1.html#_Toc66194895"^^xsd:anyURI ;
    dcat:theme legcons:Division .

F2021L00317:159 a legcons:Chapter,
        owl:Class,
        dcat:Resource ;
    rdfs:label "Chapter - C159 Chapter 8 Other matters relating to export"@en-AU ;
    dct:hasPart F2021L00317:160,
        F2021L00317:164 ;
    dct:isReferencedBy F2021L00317: ;
    rdfs:comment "Chapter 8 Other matters relating to export - Abrievated Graph Key: C159"@en-AU ;
    skos:broader F2021L00317:160,
        F2021L00317:164 ;
    skos:definition "Chapter 8 Other matters relating to export"@en-AU ;
    skos:prefLabel "Chapter C159"@en-AU ;
    dcat:accessURL <https://www.legislation.gov.au/F2021L00317/asmade/2021-03-24/text/original/epub/OEBPS/document_1/document_1.html#_Toc66194916> ;
    dcat:landingPage "https://www.legislation.gov.au/F2021L00317/asmade/2021-03-24/text/original/epub/OEBPS/document_1/document_1.html#_Toc66194916"^^xsd:anyURI ;
    dcat:theme legcons:Chapter .

F2021L00317:222 a legcons:Division,
        owl:Class,
        dcat:Resource ;
    rdfs:label "Division - D222 Division 1 General"@en-AU ;
    dct:hasPart F2021L00317:223 ;
    dct:isPartOf F2021L00317:221 ;
    dct:isReferencedBy F2021L00317: ;
    rdfs:comment "Division 1 General - Abrievated Graph Key: D222"@en-AU ;
    skos:broader F2021L00317:223 ;
    skos:definition "Division 1 General"@en-AU ;
    skos:narrower F2021L00317:221 ;
    skos:prefLabel "Division D222"@en-AU ;
    dcat:accessURL <https://www.legislation.gov.au/F2021L00317/asmade/2021-03-24/text/original/epub/OEBPS/document_1/document_1.html#_Toc66194979> ;
    dcat:landingPage "https://www.legislation.gov.au/F2021L00317/asmade/2021-03-24/text/original/epub/OEBPS/document_1/document_1.html#_Toc66194979"^^xsd:anyURI ;
    dcat:theme legcons:Division .

F2021L00317:239 a legcons:Part,
        owl:Class,
        dcat:Resource ;
    rdfs:label "Part - P239 Part 3 Powers of the Secretary"@en-AU ;
    dct:hasPart F2021L00317:240 ;
    dct:isPartOf F2021L00317:199 ;
    dct:isReferencedBy F2021L00317: ;
    rdfs:comment "Part 3 Powers of the Secretary - Abrievated Graph Key: P239"@en-AU ;
    skos:broader F2021L00317:240 ;
    skos:definition "Part 3 Powers of the Secretary"@en-AU ;
    skos:narrower F2021L00317:199 ;
    skos:prefLabel "Part P239"@en-AU ;
    dcat:accessURL <https://www.legislation.gov.au/F2021L00317/asmade/2021-03-24/text/original/epub/OEBPS/document_1/document_1.html#_Toc66194996> ;
    dcat:landingPage "https://www.legislation.gov.au/F2021L00317/asmade/2021-03-24/text/original/epub/OEBPS/document_1/document_1.html#_Toc66194996"^^xsd:anyURI ;
    dcat:theme legcons:Part .

F2021L00317:242 a legcons:Division,
        owl:Class,
        dcat:Resource ;
    rdfs:label "Division - D242 Division 1 Third party authorised officers"@en-AU ;
    dct:hasPart F2021L00317:243 ;
    dct:isPartOf F2021L00317:241 ;
    dct:isReferencedBy F2021L00317: ;
    rdfs:comment "Division 1 Third party authorised officers - Abrievated Graph Key: D242"@en-AU ;
    skos:broader F2021L00317:243 ;
    skos:definition "Division 1 Third party authorised officers"@en-AU ;
    skos:narrower F2021L00317:241 ;
    skos:prefLabel "Division D242"@en-AU ;
    dcat:accessURL <https://www.legislation.gov.au/F2021L00317/asmade/2021-03-24/text/original/epub/OEBPS/document_1/document_1.html#_Toc66194999> ;
    dcat:landingPage "https://www.legislation.gov.au/F2021L00317/asmade/2021-03-24/text/original/epub/OEBPS/document_1/document_1.html#_Toc66194999"^^xsd:anyURI ;
    dcat:theme legcons:Division .

F2021L00317:249 a legcons:Division,
        owl:Class,
        dcat:Resource ;
    rdfs:label "Division - D249 Division 3 Directions to deal with non compliance with the Act etc"@en-AU ;
    dct:hasPart F2021L00317:250 ;
    dct:isPartOf F2021L00317:241 ;
    dct:isReferencedBy F2021L00317: ;
    rdfs:comment "Division 3 Directions to deal with non compliance with the Act etc - Abrievated Graph Key: D249"@en-AU ;
    skos:broader F2021L00317:250 ;
    skos:definition "Division 3 Directions to deal with non compliance with the Act etc"@en-AU ;
    skos:narrower F2021L00317:241 ;
    skos:prefLabel "Division D249"@en-AU ;
    dcat:accessURL <https://www.legislation.gov.au/F2021L00317/asmade/2021-03-24/text/original/epub/OEBPS/document_1/document_1.html#_Toc66195006> ;
    dcat:landingPage "https://www.legislation.gov.au/F2021L00317/asmade/2021-03-24/text/original/epub/OEBPS/document_1/document_1.html#_Toc66195006"^^xsd:anyURI ;
    dcat:theme legcons:Division .

F2021L00317:251 a legcons:Division,
        owl:Class,
        dcat:Resource ;
    rdfs:label "Division - D251 Division 4 Miscellaneous"@en-AU ;
    dct:hasPart F2021L00317:252 ;
    dct:isPartOf F2021L00317:241 ;
    dct:isReferencedBy F2021L00317: ;
    rdfs:comment "Division 4 Miscellaneous - Abrievated Graph Key: D251"@en-AU ;
    skos:broader F2021L00317:252 ;
    skos:definition "Division 4 Miscellaneous"@en-AU ;
    skos:narrower F2021L00317:241 ;
    skos:prefLabel "Division D251"@en-AU ;
    dcat:accessURL <https://www.legislation.gov.au/F2021L00317/asmade/2021-03-24/text/original/epub/OEBPS/document_1/document_1.html#_Toc66195008> ;
    dcat:landingPage "https://www.legislation.gov.au/F2021L00317/asmade/2021-03-24/text/original/epub/OEBPS/document_1/document_1.html#_Toc66195008"^^xsd:anyURI ;
    dcat:theme legcons:Division .

F2021L00317:253 a legcons:Chapter,
        owl:Class,
        dcat:Resource ;
    rdfs:label "Chapter - C253 Chapter 10 Compliance and enforcement"@en-AU ;
    dct:hasPart F2021L00317:254,
        F2021L00317:255 ;
    dct:isReferencedBy F2021L00317: ;
    rdfs:comment "Chapter 10 Compliance and enforcement - Abrievated Graph Key: C253"@en-AU ;
    skos:broader F2021L00317:254,
        F2021L00317:255 ;
    skos:definition "Chapter 10 Compliance and enforcement"@en-AU ;
    skos:prefLabel "Chapter C253"@en-AU ;
    dcat:accessURL <https://www.legislation.gov.au/F2021L00317/asmade/2021-03-24/text/original/epub/OEBPS/document_1/document_1.html#_Toc66195010> ;
    dcat:landingPage "https://www.legislation.gov.au/F2021L00317/asmade/2021-03-24/text/original/epub/OEBPS/document_1/document_1.html#_Toc66195010"^^xsd:anyURI ;
    dcat:theme legcons:Chapter .

F2021L00317:257 a legcons:Part,
        owl:Class,
        dcat:Resource ;
    rdfs:label "Part - P257 Part 1 Review of decisions"@en-AU ;
    dct:hasPart F2021L00317:258 ;
    dct:isPartOf F2021L00317:256 ;
    dct:isReferencedBy F2021L00317: ;
    rdfs:comment "Part 1 Review of decisions - Abrievated Graph Key: P257"@en-AU ;
    skos:broader F2021L00317:258 ;
    skos:definition "Part 1 Review of decisions"@en-AU ;
    skos:narrower F2021L00317:256 ;
    skos:prefLabel "Part P257"@en-AU ;
    dcat:accessURL <https://www.legislation.gov.au/F2021L00317/asmade/2021-03-24/text/original/epub/OEBPS/document_1/document_1.html#_Toc66195014> ;
    dcat:landingPage "https://www.legislation.gov.au/F2021L00317/asmade/2021-03-24/text/original/epub/OEBPS/document_1/document_1.html#_Toc66195014"^^xsd:anyURI ;
    dcat:theme legcons:Part .

F2021L00317:275 a legcons:Part,
        owl:Class,
        dcat:Resource ;
    rdfs:label "Part - P275 Part 5 Relevant Commonwealth liabilities"@en-AU ;
    dct:hasPart F2021L00317:276 ;
    dct:isPartOf F2021L00317:256 ;
    dct:isReferencedBy F2021L00317: ;
    rdfs:comment "Part 5 Relevant Commonwealth liabilities - Abrievated Graph Key: P275"@en-AU ;
    skos:broader F2021L00317:276 ;
    skos:definition "Part 5 Relevant Commonwealth liabilities"@en-AU ;
    skos:narrower F2021L00317:256 ;
    skos:prefLabel "Part P275"@en-AU ;
    dcat:accessURL <https://www.legislation.gov.au/F2021L00317/asmade/2021-03-24/text/original/epub/OEBPS/document_1/document_1.html#_Toc66195032> ;
    dcat:landingPage "https://www.legislation.gov.au/F2021L00317/asmade/2021-03-24/text/original/epub/OEBPS/document_1/document_1.html#_Toc66195032"^^xsd:anyURI ;
    dcat:theme legcons:Part .

F2021L00317:278 a legcons:Part,
        owl:Class,
        dcat:Resource ;
    rdfs:label "Part - P278 Part 1 Preliminary"@en-AU ;
    dct:hasPart F2021L00317:279 ;
    dct:isPartOf F2021L00317:277 ;
    dct:isReferencedBy F2021L00317: ;
    rdfs:comment "Part 1 Preliminary - Abrievated Graph Key: P278"@en-AU ;
    skos:broader F2021L00317:279 ;
    skos:definition "Part 1 Preliminary"@en-AU ;
    skos:narrower F2021L00317:277 ;
    skos:prefLabel "Part P278"@en-AU ;
    dcat:accessURL <https://www.legislation.gov.au/F2021L00317/asmade/2021-03-24/text/original/epub/OEBPS/document_1/document_1.html#_Toc66195035> ;
    dcat:landingPage "https://www.legislation.gov.au/F2021L00317/asmade/2021-03-24/text/original/epub/OEBPS/document_1/document_1.html#_Toc66195035"^^xsd:anyURI ;
    dcat:theme legcons:Part .

F2021L00317:280 a legcons:Part,
        owl:Class,
        dcat:Resource ;
    rdfs:label "Part - P280 Part 2 Approved arrangements"@en-AU ;
    dct:hasPart F2021L00317:281 ;
    dct:isPartOf F2021L00317:277 ;
    dct:isReferencedBy F2021L00317: ;
    rdfs:comment "Part 2 Approved arrangements - Abrievated Graph Key: P280"@en-AU ;
    skos:broader F2021L00317:281 ;
    skos:definition "Part 2 Approved arrangements"@en-AU ;
    skos:narrower F2021L00317:277 ;
    skos:prefLabel "Part P280"@en-AU ;
    dcat:accessURL <https://www.legislation.gov.au/F2021L00317/asmade/2021-03-24/text/original/epub/OEBPS/document_1/document_1.html#_Toc66195037> ;
    dcat:landingPage "https://www.legislation.gov.au/F2021L00317/asmade/2021-03-24/text/original/epub/OEBPS/document_1/document_1.html#_Toc66195037"^^xsd:anyURI ;
    dcat:theme legcons:Part .

F2021L00317:283 a legcons:Division,
        owl:Class,
        dcat:Resource ;
    rdfs:label "Division - D283 Division 1 Trade descriptions"@en-AU ;
    dct:hasPart F2021L00317:284 ;
    dct:isPartOf F2021L00317:282 ;
    dct:isReferencedBy F2021L00317: ;
    rdfs:comment "Division 1 Trade descriptions - Abrievated Graph Key: D283"@en-AU ;
    skos:broader F2021L00317:284 ;
    skos:definition "Division 1 Trade descriptions"@en-AU ;
    skos:narrower F2021L00317:282 ;
    skos:prefLabel "Division D283"@en-AU ;
    dcat:accessURL <https://www.legislation.gov.au/F2021L00317/asmade/2021-03-24/text/original/epub/OEBPS/document_1/document_1.html#_Toc66195040> ;
    dcat:landingPage "https://www.legislation.gov.au/F2021L00317/asmade/2021-03-24/text/original/epub/OEBPS/document_1/document_1.html#_Toc66195040"^^xsd:anyURI ;
    dcat:theme legcons:Division .

F2021L00317:297 a legcons:Division,
        owl:Class,
        dcat:Resource ;
    rdfs:label "Division - D297 Division 2 Assessments"@en-AU ;
    dct:hasPart F2021L00317:298 ;
    dct:isPartOf F2021L00317:292 ;
    dct:isReferencedBy F2021L00317: ;
    rdfs:comment "Division 2 Assessments - Abrievated Graph Key: D297"@en-AU ;
    skos:broader F2021L00317:298 ;
    skos:definition "Division 2 Assessments"@en-AU ;
    skos:narrower F2021L00317:292 ;
    skos:prefLabel "Division D297"@en-AU ;
    dcat:accessURL <https://www.legislation.gov.au/F2021L00317/asmade/2021-03-24/text/original/epub/OEBPS/document_1/document_1.html#_Toc66195054> ;
    dcat:landingPage "https://www.legislation.gov.au/F2021L00317/asmade/2021-03-24/text/original/epub/OEBPS/document_1/document_1.html#_Toc66195054"^^xsd:anyURI ;
    dcat:theme legcons:Division .

F2021L00317:73 a legcons:Division,
        owl:Class,
        dcat:Resource ;
    rdfs:label "Division - D73 Division 1 Purpose of this Part"@en-AU ;
    dct:hasPart F2021L00317:74 ;
    dct:isPartOf F2021L00317:72 ;
    dct:isReferencedBy F2021L00317: ;
    rdfs:comment "Division 1 Purpose of this Part - Abrievated Graph Key: D73"@en-AU ;
    skos:broader F2021L00317:74 ;
    skos:definition "Division 1 Purpose of this Part"@en-AU ;
    skos:narrower F2021L00317:72 ;
    skos:prefLabel "Division D73"@en-AU ;
    dcat:accessURL <https://www.legislation.gov.au/F2021L00317/asmade/2021-03-24/text/original/epub/OEBPS/document_1/document_1.html#_Toc66194830> ;
    dcat:landingPage "https://www.legislation.gov.au/F2021L00317/asmade/2021-03-24/text/original/epub/OEBPS/document_1/document_1.html#_Toc66194830"^^xsd:anyURI ;
    dcat:theme legcons:Division .

F2021L00317:75 a legcons:Division,
        owl:Class,
        dcat:Resource ;
    rdfs:label "Division - D75 Division 2 General"@en-AU ;
    dct:hasPart F2021L00317:76 ;
    dct:isPartOf F2021L00317:72 ;
    dct:isReferencedBy F2021L00317: ;
    rdfs:comment "Division 2 General - Abrievated Graph Key: D75"@en-AU ;
    skos:broader F2021L00317:76 ;
    skos:definition "Division 2 General"@en-AU ;
    skos:narrower F2021L00317:72 ;
    skos:prefLabel "Division D75"@en-AU ;
    dcat:accessURL <https://www.legislation.gov.au/F2021L00317/asmade/2021-03-24/text/original/epub/OEBPS/document_1/document_1.html#_Toc66194832> ;
    dcat:landingPage "https://www.legislation.gov.au/F2021L00317/asmade/2021-03-24/text/original/epub/OEBPS/document_1/document_1.html#_Toc66194832"^^xsd:anyURI ;
    dcat:theme legcons:Division .

F2021L00317:13 a legcons:Division,
        owl:Class,
        dcat:Resource ;
    rdfs:label "Division - D13 Division 1 Prescribed goods"@en-AU ;
    dct:hasPart F2021L00317:14,
        F2021L00317:15 ;
    dct:isPartOf F2021L00317:12 ;
    dct:isReferencedBy F2021L00317: ;
    rdfs:comment "Division 1 Prescribed goods - Abrievated Graph Key: D13"@en-AU ;
    skos:broader F2021L00317:14,
        F2021L00317:15 ;
    skos:definition "Division 1 Prescribed goods"@en-AU ;
    skos:narrower F2021L00317:12 ;
    skos:prefLabel "Division D13"@en-AU ;
    dcat:accessURL <https://www.legislation.gov.au/F2021L00317/asmade/2021-03-24/text/original/epub/OEBPS/document_1/document_1.html#_Toc66194770> ;
    dcat:landingPage "https://www.legislation.gov.au/F2021L00317/asmade/2021-03-24/text/original/epub/OEBPS/document_1/document_1.html#_Toc66194770"^^xsd:anyURI ;
    dcat:theme legcons:Division .

F2021L00317:135 a legcons:Division,
        owl:Class,
        dcat:Resource ;
    rdfs:label "Division - D135 Division 1 Variations by holder"@en-AU ;
    dct:hasPart F2021L00317:136,
        F2021L00317:137 ;
    dct:isPartOf F2021L00317:65 ;
    dct:isReferencedBy F2021L00317: ;
    rdfs:comment "Division 1 Variations by holder - Abrievated Graph Key: D135"@en-AU ;
    skos:broader F2021L00317:136,
        F2021L00317:137 ;
    skos:definition "Division 1 Variations by holder"@en-AU ;
    skos:narrower F2021L00317:65 ;
    skos:prefLabel "Division D135"@en-AU ;
    dcat:accessURL <https://www.legislation.gov.au/F2021L00317/asmade/2021-03-24/text/original/epub/OEBPS/document_1/document_1.html#_Toc66194892> ;
    dcat:landingPage "https://www.legislation.gov.au/F2021L00317/asmade/2021-03-24/text/original/epub/OEBPS/document_1/document_1.html#_Toc66194892"^^xsd:anyURI ;
    dcat:theme legcons:Division .

F2021L00317:145 a legcons:Part,
        owl:Class,
        dcat:Resource ;
    rdfs:label "Part - P145 Part 1 Issue of export permit"@en-AU ;
    dct:hasPart F2021L00317:146,
        F2021L00317:147 ;
    dct:isPartOf F2021L00317:144 ;
    dct:isReferencedBy F2021L00317: ;
    rdfs:comment "Part 1 Issue of export permit - Abrievated Graph Key: P145"@en-AU ;
    skos:broader F2021L00317:146,
        F2021L00317:147 ;
    skos:definition "Part 1 Issue of export permit"@en-AU ;
    skos:narrower F2021L00317:144 ;
    skos:prefLabel "Part P145"@en-AU ;
    dcat:accessURL <https://www.legislation.gov.au/F2021L00317/asmade/2021-03-24/text/original/epub/OEBPS/document_1/document_1.html#_Toc66194902> ;
    dcat:landingPage "https://www.legislation.gov.au/F2021L00317/asmade/2021-03-24/text/original/epub/OEBPS/document_1/document_1.html#_Toc66194902"^^xsd:anyURI ;
    dcat:theme legcons:Part .

F2021L00317:156 a legcons:Part,
        owl:Class,
        dcat:Resource ;
    rdfs:label "Part - P156 Part 4 Applications for export permits"@en-AU ;
    dct:hasPart F2021L00317:157,
        F2021L00317:158 ;
    dct:isPartOf F2021L00317:144 ;
    dct:isReferencedBy F2021L00317: ;
    rdfs:comment "Part 4 Applications for export permits - Abrievated Graph Key: P156"@en-AU ;
    skos:broader F2021L00317:157,
        F2021L00317:158 ;
    skos:definition "Part 4 Applications for export permits"@en-AU ;
    skos:narrower F2021L00317:144 ;
    skos:prefLabel "Part P156"@en-AU ;
    dcat:accessURL <https://www.legislation.gov.au/F2021L00317/asmade/2021-03-24/text/original/epub/OEBPS/document_1/document_1.html#_Toc66194913> ;
    dcat:landingPage "https://www.legislation.gov.au/F2021L00317/asmade/2021-03-24/text/original/epub/OEBPS/document_1/document_1.html#_Toc66194913"^^xsd:anyURI ;
    dcat:theme legcons:Part .

F2021L00317:201 a legcons:Division,
        owl:Class,
        dcat:Resource ;
    rdfs:label "Division - D201 Division 1 General"@en-AU ;
    dct:hasPart F2021L00317:202,
        F2021L00317:203 ;
    dct:isPartOf F2021L00317:200 ;
    dct:isReferencedBy F2021L00317: ;
    rdfs:comment "Division 1 General - Abrievated Graph Key: D201"@en-AU ;
    skos:broader F2021L00317:202,
        F2021L00317:203 ;
    skos:definition "Division 1 General"@en-AU ;
    skos:narrower F2021L00317:200 ;
    skos:prefLabel "Division D201"@en-AU ;
    dcat:accessURL <https://www.legislation.gov.au/F2021L00317/asmade/2021-03-24/text/original/epub/OEBPS/document_1/document_1.html#_Toc66194958> ;
    dcat:landingPage "https://www.legislation.gov.au/F2021L00317/asmade/2021-03-24/text/original/epub/OEBPS/document_1/document_1.html#_Toc66194958"^^xsd:anyURI ;
    dcat:theme legcons:Division .

F2021L00317:224 a legcons:Division,
        owl:Class,
        dcat:Resource ;
    rdfs:label "Division - D224 Division 2 Carrying out assessments etc"@en-AU ;
    dct:hasPart F2021L00317:225,
        F2021L00317:226 ;
    dct:isPartOf F2021L00317:221 ;
    dct:isReferencedBy F2021L00317: ;
    rdfs:comment "Division 2 Carrying out assessments etc - Abrievated Graph Key: D224"@en-AU ;
    skos:broader F2021L00317:225,
        F2021L00317:226 ;
    skos:definition "Division 2 Carrying out assessments etc"@en-AU ;
    skos:narrower F2021L00317:221 ;
    skos:prefLabel "Division D224"@en-AU ;
    dcat:accessURL <https://www.legislation.gov.au/F2021L00317/asmade/2021-03-24/text/original/epub/OEBPS/document_1/document_1.html#_Toc66194981> ;
    dcat:landingPage "https://www.legislation.gov.au/F2021L00317/asmade/2021-03-24/text/original/epub/OEBPS/document_1/document_1.html#_Toc66194981"^^xsd:anyURI ;
    dcat:theme legcons:Division .

F2021L00317:269 a legcons:Part,
        owl:Class,
        dcat:Resource ;
    rdfs:label "Part - P269 Part 3 Samples"@en-AU ;
    dct:hasPart F2021L00317:270,
        F2021L00317:271 ;
    dct:isPartOf F2021L00317:256 ;
    dct:isReferencedBy F2021L00317: ;
    rdfs:comment "Part 3 Samples - Abrievated Graph Key: P269"@en-AU ;
    skos:broader F2021L00317:270,
        F2021L00317:271 ;
    skos:definition "Part 3 Samples"@en-AU ;
    skos:narrower F2021L00317:256 ;
    skos:prefLabel "Part P269"@en-AU ;
    dcat:accessURL <https://www.legislation.gov.au/F2021L00317/asmade/2021-03-24/text/original/epub/OEBPS/document_1/document_1.html#_Toc66195026> ;
    dcat:landingPage "https://www.legislation.gov.au/F2021L00317/asmade/2021-03-24/text/original/epub/OEBPS/document_1/document_1.html#_Toc66195026"^^xsd:anyURI ;
    dcat:theme legcons:Part .

F2021L00317:272 a legcons:Part,
        owl:Class,
        dcat:Resource ;
    rdfs:label "Part - P272 Part 4 Damaged or destroyed fish or fish products"@en-AU ;
    dct:hasPart F2021L00317:273,
        F2021L00317:274 ;
    dct:isPartOf F2021L00317:256 ;
    dct:isReferencedBy F2021L00317: ;
    rdfs:comment "Part 4 Damaged or destroyed fish or fish products - Abrievated Graph Key: P272"@en-AU ;
    skos:broader F2021L00317:273,
        F2021L00317:274 ;
    skos:definition "Part 4 Damaged or destroyed fish or fish products"@en-AU ;
    skos:narrower F2021L00317:256 ;
    skos:prefLabel "Part P272"@en-AU ;
    dcat:accessURL <https://www.legislation.gov.au/F2021L00317/asmade/2021-03-24/text/original/epub/OEBPS/document_1/document_1.html#_Toc66195029> ;
    dcat:landingPage "https://www.legislation.gov.au/F2021L00317/asmade/2021-03-24/text/original/epub/OEBPS/document_1/document_1.html#_Toc66195029"^^xsd:anyURI ;
    dcat:theme legcons:Part .

F2021L00317:289 a legcons:Division,
        owl:Class,
        dcat:Resource ;
    rdfs:label "Division - D289 Division 3 Official marking devices"@en-AU ;
    dct:hasPart F2021L00317:290,
        F2021L00317:291 ;
    dct:isPartOf F2021L00317:282 ;
    dct:isReferencedBy F2021L00317: ;
    rdfs:comment "Division 3 Official marking devices - Abrievated Graph Key: D289"@en-AU ;
    skos:broader F2021L00317:290,
        F2021L00317:291 ;
    skos:definition "Division 3 Official marking devices"@en-AU ;
    skos:narrower F2021L00317:282 ;
    skos:prefLabel "Division D289"@en-AU ;
    dcat:accessURL <https://www.legislation.gov.au/F2021L00317/asmade/2021-03-24/text/original/epub/OEBPS/document_1/document_1.html#_Toc66195046> ;
    dcat:landingPage "https://www.legislation.gov.au/F2021L00317/asmade/2021-03-24/text/original/epub/OEBPS/document_1/document_1.html#_Toc66195046"^^xsd:anyURI ;
    dcat:theme legcons:Division .

F2021L00317:292 a legcons:Part,
        owl:Class,
        dcat:Resource ;
    rdfs:label "Part - P292 Part 4 Powers and officials"@en-AU ;
    dct:hasPart F2021L00317:293,
        F2021L00317:297 ;
    dct:isPartOf F2021L00317:277 ;
    dct:isReferencedBy F2021L00317: ;
    rdfs:comment "Part 4 Powers and officials - Abrievated Graph Key: P292"@en-AU ;
    skos:broader F2021L00317:293,
        F2021L00317:297 ;
    skos:definition "Part 4 Powers and officials"@en-AU ;
    skos:narrower F2021L00317:277 ;
    skos:prefLabel "Part P292"@en-AU ;
    dcat:accessURL <https://www.legislation.gov.au/F2021L00317/asmade/2021-03-24/text/original/epub/OEBPS/document_1/document_1.html#_Toc66195049> ;
    dcat:landingPage "https://www.legislation.gov.au/F2021L00317/asmade/2021-03-24/text/original/epub/OEBPS/document_1/document_1.html#_Toc66195049"^^xsd:anyURI ;
    dcat:theme legcons:Part .

F2021L00317:36 a legcons:Part,
        owl:Class,
        dcat:Resource ;
    rdfs:label "Part - P36 Part 1 Requirements for registration"@en-AU ;
    dct:hasPart F2021L00317:37,
        F2021L00317:48 ;
    dct:isPartOf F2021L00317:35 ;
    dct:isReferencedBy F2021L00317: ;
    rdfs:comment "Part 1 Requirements for registration - Abrievated Graph Key: P36"@en-AU ;
    skos:broader F2021L00317:37,
        F2021L00317:48 ;
    skos:definition "Part 1 Requirements for registration"@en-AU ;
    skos:narrower F2021L00317:35 ;
    skos:prefLabel "Part P36"@en-AU ;
    dcat:accessURL <https://www.legislation.gov.au/F2021L00317/asmade/2021-03-24/text/original/epub/OEBPS/document_1/document_1.html#_Toc66194793> ;
    dcat:landingPage "https://www.legislation.gov.au/F2021L00317/asmade/2021-03-24/text/original/epub/OEBPS/document_1/document_1.html#_Toc66194793"^^xsd:anyURI ;
    dcat:theme legcons:Part .

F2021L00317:48 a legcons:Division,
        owl:Class,
        dcat:Resource ;
    rdfs:label "Division - D48 Division 2 Other requirements"@en-AU ;
    dct:hasPart F2021L00317:49,
        F2021L00317:50 ;
    dct:isPartOf F2021L00317:36 ;
    dct:isReferencedBy F2021L00317: ;
    rdfs:comment "Division 2 Other requirements - Abrievated Graph Key: D48"@en-AU ;
    skos:broader F2021L00317:49,
        F2021L00317:50 ;
    skos:definition "Division 2 Other requirements"@en-AU ;
    skos:narrower F2021L00317:36 ;
    skos:prefLabel "Division D48"@en-AU ;
    dcat:accessURL <https://www.legislation.gov.au/F2021L00317/asmade/2021-03-24/text/original/epub/OEBPS/document_1/document_1.html#_Toc66194805> ;
    dcat:landingPage "https://www.legislation.gov.au/F2021L00317/asmade/2021-03-24/text/original/epub/OEBPS/document_1/document_1.html#_Toc66194805"^^xsd:anyURI ;
    dcat:theme legcons:Division .

F2021L00317:55 a legcons:Part,
        owl:Class,
        dcat:Resource ;
    rdfs:label "Part - P55 Part 3 Renewal of registration"@en-AU ;
    dct:hasPart F2021L00317:56,
        F2021L00317:57 ;
    dct:isPartOf F2021L00317:35 ;
    dct:isReferencedBy F2021L00317: ;
    rdfs:comment "Part 3 Renewal of registration - Abrievated Graph Key: P55"@en-AU ;
    skos:broader F2021L00317:56,
        F2021L00317:57 ;
    skos:definition "Part 3 Renewal of registration"@en-AU ;
    skos:narrower F2021L00317:35 ;
    skos:prefLabel "Part P55"@en-AU ;
    dcat:accessURL <https://www.legislation.gov.au/F2021L00317/asmade/2021-03-24/text/original/epub/OEBPS/document_1/document_1.html#_Toc66194812> ;
    dcat:landingPage "https://www.legislation.gov.au/F2021L00317/asmade/2021-03-24/text/original/epub/OEBPS/document_1/document_1.html#_Toc66194812"^^xsd:anyURI ;
    dcat:theme legcons:Part .

F2021L00317:58 a legcons:Part,
        owl:Class,
        dcat:Resource ;
    rdfs:label "Part - P58 Part 4 Suspension of registration"@en-AU ;
    dct:hasPart F2021L00317:59,
        F2021L00317:60 ;
    dct:isPartOf F2021L00317:35 ;
    dct:isReferencedBy F2021L00317: ;
    rdfs:comment "Part 4 Suspension of registration - Abrievated Graph Key: P58"@en-AU ;
    skos:broader F2021L00317:59,
        F2021L00317:60 ;
    skos:definition "Part 4 Suspension of registration"@en-AU ;
    skos:narrower F2021L00317:35 ;
    skos:prefLabel "Part P58"@en-AU ;
    dcat:accessURL <https://www.legislation.gov.au/F2021L00317/asmade/2021-03-24/text/original/epub/OEBPS/document_1/document_1.html#_Toc66194815> ;
    dcat:landingPage "https://www.legislation.gov.au/F2021L00317/asmade/2021-03-24/text/original/epub/OEBPS/document_1/document_1.html#_Toc66194815"^^xsd:anyURI ;
    dcat:theme legcons:Part .

F2021L00317:103 a legcons:Subdivision,
        owl:Class,
        dcat:Resource ;
    rdfs:label "Subdivision - S103 Subdivision BShellfish"@en-AU ;
    dct:hasPart F2021L00317:104,
        F2021L00317:105,
        F2021L00317:106 ;
    dct:isPartOf F2021L00317:72 ;
    dct:isReferencedBy F2021L00317: ;
    rdfs:comment "Subdivision BShellfish - Abrievated Graph Key: S103"@en-AU ;
    skos:broader F2021L00317:104,
        F2021L00317:105,
        F2021L00317:106 ;
    skos:definition "Subdivision BShellfish"@en-AU ;
    skos:narrower F2021L00317:72 ;
    skos:prefLabel "Subdivision S103"@en-AU ;
    dcat:accessURL <https://www.legislation.gov.au/F2021L00317/asmade/2021-03-24/text/original/epub/OEBPS/document_1/document_1.html#_Toc66194860> ;
    dcat:landingPage "https://www.legislation.gov.au/F2021L00317/asmade/2021-03-24/text/original/epub/OEBPS/document_1/document_1.html#_Toc66194860"^^xsd:anyURI ;
    dcat:theme legcons:Subdivision .

F2021L00317:107 a legcons:Subdivision,
        owl:Class,
        dcat:Resource ;
    rdfs:label "Subdivision - S107 Subdivision CCrocodiles and crocodile meat"@en-AU ;
    dct:hasPart F2021L00317:108,
        F2021L00317:109,
        F2021L00317:110 ;
    dct:isPartOf F2021L00317:72 ;
    dct:isReferencedBy F2021L00317: ;
    rdfs:comment "Subdivision CCrocodiles and crocodile meat - Abrievated Graph Key: S107"@en-AU ;
    skos:broader F2021L00317:108,
        F2021L00317:109,
        F2021L00317:110 ;
    skos:definition "Subdivision CCrocodiles and crocodile meat"@en-AU ;
    skos:narrower F2021L00317:72 ;
    skos:prefLabel "Subdivision S107"@en-AU ;
    dcat:accessURL <https://www.legislation.gov.au/F2021L00317/asmade/2021-03-24/text/original/epub/OEBPS/document_1/document_1.html#_Toc66194864> ;
    dcat:landingPage "https://www.legislation.gov.au/F2021L00317/asmade/2021-03-24/text/original/epub/OEBPS/document_1/document_1.html#_Toc66194864"^^xsd:anyURI ;
    dcat:theme legcons:Subdivision .

F2021L00317:144 a legcons:Chapter,
        owl:Class,
        dcat:Resource ;
    rdfs:label "Chapter - C144 Chapter 7 Export permits"@en-AU ;
    dct:hasPart F2021L00317:145,
        F2021L00317:148,
        F2021L00317:152,
        F2021L00317:156 ;
    dct:isReferencedBy F2021L00317: ;
    rdfs:comment "Chapter 7 Export permits - Abrievated Graph Key: C144"@en-AU ;
    skos:broader F2021L00317:145,
        F2021L00317:148,
        F2021L00317:152,
        F2021L00317:156 ;
    skos:definition "Chapter 7 Export permits"@en-AU ;
    skos:prefLabel "Chapter C144"@en-AU ;
    dcat:accessURL <https://www.legislation.gov.au/F2021L00317/asmade/2021-03-24/text/original/epub/OEBPS/document_1/document_1.html#_Toc66194901> ;
    dcat:landingPage "https://www.legislation.gov.au/F2021L00317/asmade/2021-03-24/text/original/epub/OEBPS/document_1/document_1.html#_Toc66194901"^^xsd:anyURI ;
    dcat:theme legcons:Chapter .

F2021L00317:148 a legcons:Part,
        owl:Class,
        dcat:Resource ;
    rdfs:label "Part - P148 Part 2 Variation suspension and revocation of export permit"@en-AU ;
    dct:hasPart F2021L00317:149,
        F2021L00317:150,
        F2021L00317:151 ;
    dct:isPartOf F2021L00317:144 ;
    dct:isReferencedBy F2021L00317: ;
    rdfs:comment "Part 2 Variation suspension and revocation of export permit - Abrievated Graph Key: P148"@en-AU ;
    skos:broader F2021L00317:149,
        F2021L00317:150,
        F2021L00317:151 ;
    skos:definition "Part 2 Variation suspension and revocation of export permit"@en-AU ;
    skos:narrower F2021L00317:144 ;
    skos:prefLabel "Part P148"@en-AU ;
    dcat:accessURL <https://www.legislation.gov.au/F2021L00317/asmade/2021-03-24/text/original/epub/OEBPS/document_1/document_1.html#_Toc66194905> ;
    dcat:landingPage "https://www.legislation.gov.au/F2021L00317/asmade/2021-03-24/text/original/epub/OEBPS/document_1/document_1.html#_Toc66194905"^^xsd:anyURI ;
    dcat:theme legcons:Part .

F2021L00317:152 a legcons:Part,
        owl:Class,
        dcat:Resource ;
    rdfs:label "Part - P152 Part 3 Other matters"@en-AU ;
    dct:hasPart F2021L00317:153,
        F2021L00317:154,
        F2021L00317:155 ;
    dct:isPartOf F2021L00317:144 ;
    dct:isReferencedBy F2021L00317: ;
    rdfs:comment "Part 3 Other matters - Abrievated Graph Key: P152"@en-AU ;
    skos:broader F2021L00317:153,
        F2021L00317:154,
        F2021L00317:155 ;
    skos:definition "Part 3 Other matters"@en-AU ;
    skos:narrower F2021L00317:144 ;
    skos:prefLabel "Part P152"@en-AU ;
    dcat:accessURL <https://www.legislation.gov.au/F2021L00317/asmade/2021-03-24/text/original/epub/OEBPS/document_1/document_1.html#_Toc66194909> ;
    dcat:landingPage "https://www.legislation.gov.au/F2021L00317/asmade/2021-03-24/text/original/epub/OEBPS/document_1/document_1.html#_Toc66194909"^^xsd:anyURI ;
    dcat:theme legcons:Part .

F2021L00317:160 a legcons:Part,
        owl:Class,
        dcat:Resource ;
    rdfs:label "Part - P160 Part 1 Trade descriptions"@en-AU ;
    dct:hasPart F2021L00317:161,
        F2021L00317:162,
        F2021L00317:163 ;
    dct:isPartOf F2021L00317:159 ;
    dct:isReferencedBy F2021L00317: ;
    rdfs:comment "Part 1 Trade descriptions - Abrievated Graph Key: P160"@en-AU ;
    skos:broader F2021L00317:161,
        F2021L00317:162,
        F2021L00317:163 ;
    skos:definition "Part 1 Trade descriptions"@en-AU ;
    skos:narrower F2021L00317:159 ;
    skos:prefLabel "Part P160"@en-AU ;
    dcat:accessURL <https://www.legislation.gov.au/F2021L00317/asmade/2021-03-24/text/original/epub/OEBPS/document_1/document_1.html#_Toc66194917> ;
    dcat:landingPage "https://www.legislation.gov.au/F2021L00317/asmade/2021-03-24/text/original/epub/OEBPS/document_1/document_1.html#_Toc66194917"^^xsd:anyURI ;
    dcat:theme legcons:Part .

F2021L00317:188 a legcons:Division,
        owl:Class,
        dcat:Resource ;
    rdfs:label "Division - D188 Division 3 Marks resembling official marks"@en-AU ;
    dct:hasPart F2021L00317:189,
        F2021L00317:190,
        F2021L00317:191 ;
    dct:isPartOf F2021L00317:164 ;
    dct:isReferencedBy F2021L00317: ;
    rdfs:comment "Division 3 Marks resembling official marks - Abrievated Graph Key: D188"@en-AU ;
    skos:broader F2021L00317:189,
        F2021L00317:190,
        F2021L00317:191 ;
    skos:definition "Division 3 Marks resembling official marks"@en-AU ;
    skos:narrower F2021L00317:164 ;
    skos:prefLabel "Division D188"@en-AU ;
    dcat:accessURL <https://www.legislation.gov.au/F2021L00317/asmade/2021-03-24/text/original/epub/OEBPS/document_1/document_1.html#_Toc66194945> ;
    dcat:landingPage "https://www.legislation.gov.au/F2021L00317/asmade/2021-03-24/text/original/epub/OEBPS/document_1/document_1.html#_Toc66194945"^^xsd:anyURI ;
    dcat:theme legcons:Division .

F2021L00317:199 a legcons:Chapter,
        owl:Class,
        dcat:Resource ;
    rdfs:label "Chapter - C199 Chapter 9 Powers and officials"@en-AU ;
    dct:hasPart F2021L00317:200,
        F2021L00317:221,
        F2021L00317:239,
        F2021L00317:241 ;
    dct:isReferencedBy F2021L00317: ;
    rdfs:comment "Chapter 9 Powers and officials - Abrievated Graph Key: C199"@en-AU ;
    skos:broader F2021L00317:200,
        F2021L00317:221,
        F2021L00317:239,
        F2021L00317:241 ;
    skos:definition "Chapter 9 Powers and officials"@en-AU ;
    skos:prefLabel "Chapter C199"@en-AU ;
    dcat:accessURL <https://www.legislation.gov.au/F2021L00317/asmade/2021-03-24/text/original/epub/OEBPS/document_1/document_1.html#_Toc66194956> ;
    dcat:landingPage "https://www.legislation.gov.au/F2021L00317/asmade/2021-03-24/text/original/epub/OEBPS/document_1/document_1.html#_Toc66194956"^^xsd:anyURI ;
    dcat:theme legcons:Chapter .

F2021L00317:200 a legcons:Part,
        owl:Class,
        dcat:Resource ;
    rdfs:label "Part - P200 Part 1 Audits"@en-AU ;
    dct:hasPart F2021L00317:201,
        F2021L00317:204,
        F2021L00317:209 ;
    dct:isPartOf F2021L00317:199 ;
    dct:isReferencedBy F2021L00317: ;
    rdfs:comment "Part 1 Audits - Abrievated Graph Key: P200"@en-AU ;
    skos:broader F2021L00317:201,
        F2021L00317:204,
        F2021L00317:209 ;
    skos:definition "Part 1 Audits"@en-AU ;
    skos:narrower F2021L00317:199 ;
    skos:prefLabel "Part P200"@en-AU ;
    dcat:accessURL <https://www.legislation.gov.au/F2021L00317/asmade/2021-03-24/text/original/epub/OEBPS/document_1/document_1.html#_Toc66194957> ;
    dcat:landingPage "https://www.legislation.gov.au/F2021L00317/asmade/2021-03-24/text/original/epub/OEBPS/document_1/document_1.html#_Toc66194957"^^xsd:anyURI ;
    dcat:theme legcons:Part .

F2021L00317:221 a legcons:Part,
        owl:Class,
        dcat:Resource ;
    rdfs:label "Part - P221 Part 2 Assessments"@en-AU ;
    dct:hasPart F2021L00317:222,
        F2021L00317:224,
        F2021L00317:227 ;
    dct:isPartOf F2021L00317:199 ;
    dct:isReferencedBy F2021L00317: ;
    rdfs:comment "Part 2 Assessments - Abrievated Graph Key: P221"@en-AU ;
    skos:broader F2021L00317:222,
        F2021L00317:224,
        F2021L00317:227 ;
    skos:definition "Part 2 Assessments"@en-AU ;
    skos:narrower F2021L00317:199 ;
    skos:prefLabel "Part P221"@en-AU ;
    dcat:accessURL <https://www.legislation.gov.au/F2021L00317/asmade/2021-03-24/text/original/epub/OEBPS/document_1/document_1.html#_Toc66194978> ;
    dcat:landingPage "https://www.legislation.gov.au/F2021L00317/asmade/2021-03-24/text/original/epub/OEBPS/document_1/document_1.html#_Toc66194978"^^xsd:anyURI ;
    dcat:theme legcons:Part .

F2021L00317:277 a legcons:Chapter,
        owl:Class,
        dcat:Resource ;
    rdfs:label "Chapter - C277 Chapter 12 Transitional provisions"@en-AU ;
    dct:hasPart F2021L00317:278,
        F2021L00317:280,
        F2021L00317:282,
        F2021L00317:292 ;
    dct:isReferencedBy F2021L00317: ;
    rdfs:comment "Chapter 12 Transitional provisions - Abrievated Graph Key: C277"@en-AU ;
    skos:broader F2021L00317:278,
        F2021L00317:280,
        F2021L00317:282,
        F2021L00317:292 ;
    skos:definition "Chapter 12 Transitional provisions"@en-AU ;
    skos:prefLabel "Chapter C277"@en-AU ;
    dcat:accessURL <https://www.legislation.gov.au/F2021L00317/asmade/2021-03-24/text/original/epub/OEBPS/document_1/document_1.html#_Toc66195034> ;
    dcat:landingPage "https://www.legislation.gov.au/F2021L00317/asmade/2021-03-24/text/original/epub/OEBPS/document_1/document_1.html#_Toc66195034"^^xsd:anyURI ;
    dcat:theme legcons:Chapter .

F2021L00317:282 a legcons:Part,
        owl:Class,
        dcat:Resource ;
    rdfs:label "Part - P282 Part 3 Other matters relating to export"@en-AU ;
    dct:hasPart F2021L00317:283,
        F2021L00317:285,
        F2021L00317:289 ;
    dct:isPartOf F2021L00317:277 ;
    dct:isReferencedBy F2021L00317: ;
    rdfs:comment "Part 3 Other matters relating to export - Abrievated Graph Key: P282"@en-AU ;
    skos:broader F2021L00317:283,
        F2021L00317:285,
        F2021L00317:289 ;
    skos:definition "Part 3 Other matters relating to export"@en-AU ;
    skos:narrower F2021L00317:277 ;
    skos:prefLabel "Part P282"@en-AU ;
    dcat:accessURL <https://www.legislation.gov.au/F2021L00317/asmade/2021-03-24/text/original/epub/OEBPS/document_1/document_1.html#_Toc66195039> ;
    dcat:landingPage "https://www.legislation.gov.au/F2021L00317/asmade/2021-03-24/text/original/epub/OEBPS/document_1/document_1.html#_Toc66195039"^^xsd:anyURI ;
    dcat:theme legcons:Part .

F2021L00317:285 a legcons:Division,
        owl:Class,
        dcat:Resource ;
    rdfs:label "Division - D285 Division 2 Official marks"@en-AU ;
    dct:hasPart F2021L00317:286,
        F2021L00317:287,
        F2021L00317:288 ;
    dct:isPartOf F2021L00317:282 ;
    dct:isReferencedBy F2021L00317: ;
    rdfs:comment "Division 2 Official marks - Abrievated Graph Key: D285"@en-AU ;
    skos:broader F2021L00317:286,
        F2021L00317:287,
        F2021L00317:288 ;
    skos:definition "Division 2 Official marks"@en-AU ;
    skos:narrower F2021L00317:282 ;
    skos:prefLabel "Division D285"@en-AU ;
    dcat:accessURL <https://www.legislation.gov.au/F2021L00317/asmade/2021-03-24/text/original/epub/OEBPS/document_1/document_1.html#_Toc66195042> ;
    dcat:landingPage "https://www.legislation.gov.au/F2021L00317/asmade/2021-03-24/text/original/epub/OEBPS/document_1/document_1.html#_Toc66195042"^^xsd:anyURI ;
    dcat:theme legcons:Division .

F2021L00317:293 a legcons:Division,
        owl:Class,
        dcat:Resource ;
    rdfs:label "Division - D293 Division 1 Approved auditors"@en-AU ;
    dct:hasPart F2021L00317:294,
        F2021L00317:295,
        F2021L00317:296 ;
    dct:isPartOf F2021L00317:292 ;
    dct:isReferencedBy F2021L00317: ;
    rdfs:comment "Division 1 Approved auditors - Abrievated Graph Key: D293"@en-AU ;
    skos:broader F2021L00317:294,
        F2021L00317:295,
        F2021L00317:296 ;
    skos:definition "Division 1 Approved auditors"@en-AU ;
    skos:narrower F2021L00317:292 ;
    skos:prefLabel "Division D293"@en-AU ;
    dcat:accessURL <https://www.legislation.gov.au/F2021L00317/asmade/2021-03-24/text/original/epub/OEBPS/document_1/document_1.html#_Toc66195050> ;
    dcat:landingPage "https://www.legislation.gov.au/F2021L00317/asmade/2021-03-24/text/original/epub/OEBPS/document_1/document_1.html#_Toc66195050"^^xsd:anyURI ;
    dcat:theme legcons:Division .

F2021L00317:51 a legcons:Part,
        owl:Class,
        dcat:Resource ;
    rdfs:label "Part - P51 Part 2 Conditions of registration"@en-AU ;
    dct:hasPart F2021L00317:52,
        F2021L00317:53,
        F2021L00317:54 ;
    dct:isPartOf F2021L00317:35 ;
    dct:isReferencedBy F2021L00317: ;
    rdfs:comment "Part 2 Conditions of registration - Abrievated Graph Key: P51"@en-AU ;
    skos:broader F2021L00317:52,
        F2021L00317:53,
        F2021L00317:54 ;
    skos:definition "Part 2 Conditions of registration"@en-AU ;
    skos:narrower F2021L00317:35 ;
    skos:prefLabel "Part P51"@en-AU ;
    dcat:accessURL <https://www.legislation.gov.au/F2021L00317/asmade/2021-03-24/text/original/epub/OEBPS/document_1/document_1.html#_Toc66194808> ;
    dcat:landingPage "https://www.legislation.gov.au/F2021L00317/asmade/2021-03-24/text/original/epub/OEBPS/document_1/document_1.html#_Toc66194808"^^xsd:anyURI ;
    dcat:theme legcons:Part .

F2021L00317:61 a legcons:Part,
        owl:Class,
        dcat:Resource ;
    rdfs:label "Part - P61 Part 5 Matters relating to applications"@en-AU ;
    dct:hasPart F2021L00317:62,
        F2021L00317:63,
        F2021L00317:64 ;
    dct:isPartOf F2021L00317:35 ;
    dct:isReferencedBy F2021L00317: ;
    rdfs:comment "Part 5 Matters relating to applications - Abrievated Graph Key: P61"@en-AU ;
    skos:broader F2021L00317:62,
        F2021L00317:63,
        F2021L00317:64 ;
    skos:definition "Part 5 Matters relating to applications"@en-AU ;
    skos:narrower F2021L00317:35 ;
    skos:prefLabel "Part P61"@en-AU ;
    dcat:accessURL <https://www.legislation.gov.au/F2021L00317/asmade/2021-03-24/text/original/epub/OEBPS/document_1/document_1.html#_Toc66194818> ;
    dcat:landingPage "https://www.legislation.gov.au/F2021L00317/asmade/2021-03-24/text/original/epub/OEBPS/document_1/document_1.html#_Toc66194818"^^xsd:anyURI ;
    dcat:theme legcons:Part .

F2021L00317:12 a legcons:Part,
        owl:Class,
        dcat:Resource ;
    rdfs:label "Part - P12 Part 1 Goods"@en-AU ;
    dct:hasPart F2021L00317:13,
        F2021L00317:16,
        F2021L00317:17,
        F2021L00317:18 ;
    dct:isPartOf F2021L00317:11 ;
    dct:isReferencedBy F2021L00317: ;
    rdfs:comment "Part 1 Goods - Abrievated Graph Key: P12"@en-AU ;
    skos:broader F2021L00317:13,
        F2021L00317:16,
        F2021L00317:17,
        F2021L00317:18 ;
    skos:definition "Part 1 Goods"@en-AU ;
    skos:narrower F2021L00317:11 ;
    skos:prefLabel "Part P12"@en-AU ;
    dcat:accessURL <https://www.legislation.gov.au/F2021L00317/asmade/2021-03-24/text/original/epub/OEBPS/document_1/document_1.html#_Toc66194769> ;
    dcat:landingPage "https://www.legislation.gov.au/F2021L00317/asmade/2021-03-24/text/original/epub/OEBPS/document_1/document_1.html#_Toc66194769"^^xsd:anyURI ;
    dcat:theme legcons:Part .

F2021L00317:164 a legcons:Part,
        owl:Class,
        dcat:Resource ;
    rdfs:label "Part - P164 Part 2 Official marks"@en-AU ;
    dct:hasPart F2021L00317:165,
        F2021L00317:175,
        F2021L00317:188,
        F2021L00317:192 ;
    dct:isPartOf F2021L00317:159 ;
    dct:isReferencedBy F2021L00317: ;
    rdfs:comment "Part 2 Official marks - Abrievated Graph Key: P164"@en-AU ;
    skos:broader F2021L00317:165,
        F2021L00317:175,
        F2021L00317:188,
        F2021L00317:192 ;
    skos:definition "Part 2 Official marks"@en-AU ;
    skos:narrower F2021L00317:159 ;
    skos:prefLabel "Part P164"@en-AU ;
    dcat:accessURL <https://www.legislation.gov.au/F2021L00317/asmade/2021-03-24/text/original/epub/OEBPS/document_1/document_1.html#_Toc66194921> ;
    dcat:landingPage "https://www.legislation.gov.au/F2021L00317/asmade/2021-03-24/text/original/epub/OEBPS/document_1/document_1.html#_Toc66194921"^^xsd:anyURI ;
    dcat:theme legcons:Part .

F2021L00317:204 a legcons:Division,
        owl:Class,
        dcat:Resource ;
    rdfs:label "Division - D204 Division 2 Conduct of audit etc"@en-AU ;
    dct:hasPart F2021L00317:205,
        F2021L00317:206,
        F2021L00317:207,
        F2021L00317:208 ;
    dct:isPartOf F2021L00317:200 ;
    dct:isReferencedBy F2021L00317: ;
    rdfs:comment "Division 2 Conduct of audit etc - Abrievated Graph Key: D204"@en-AU ;
    skos:broader F2021L00317:205,
        F2021L00317:206,
        F2021L00317:207,
        F2021L00317:208 ;
    skos:definition "Division 2 Conduct of audit etc"@en-AU ;
    skos:narrower F2021L00317:200 ;
    skos:prefLabel "Division D204"@en-AU ;
    dcat:accessURL <https://www.legislation.gov.au/F2021L00317/asmade/2021-03-24/text/original/epub/OEBPS/document_1/document_1.html#_Toc66194961> ;
    dcat:landingPage "https://www.legislation.gov.au/F2021L00317/asmade/2021-03-24/text/original/epub/OEBPS/document_1/document_1.html#_Toc66194961"^^xsd:anyURI ;
    dcat:theme legcons:Division .

F2021L00317:241 a legcons:Part,
        owl:Class,
        dcat:Resource ;
    rdfs:label "Part - P241 Part 4 Authorised officers"@en-AU ;
    dct:hasPart F2021L00317:242,
        F2021L00317:244,
        F2021L00317:249,
        F2021L00317:251 ;
    dct:isPartOf F2021L00317:199 ;
    dct:isReferencedBy F2021L00317: ;
    rdfs:comment "Part 4 Authorised officers - Abrievated Graph Key: P241"@en-AU ;
    skos:broader F2021L00317:242,
        F2021L00317:244,
        F2021L00317:249,
        F2021L00317:251 ;
    skos:definition "Part 4 Authorised officers"@en-AU ;
    skos:narrower F2021L00317:199 ;
    skos:prefLabel "Part P241"@en-AU ;
    dcat:accessURL <https://www.legislation.gov.au/F2021L00317/asmade/2021-03-24/text/original/epub/OEBPS/document_1/document_1.html#_Toc66194998> ;
    dcat:landingPage "https://www.legislation.gov.au/F2021L00317/asmade/2021-03-24/text/original/epub/OEBPS/document_1/document_1.html#_Toc66194998"^^xsd:anyURI ;
    dcat:theme legcons:Part .

F2021L00317:244 a legcons:Division,
        owl:Class,
        dcat:Resource ;
    rdfs:label "Division - D244 Division 2 Functions and powers"@en-AU ;
    dct:hasPart F2021L00317:245,
        F2021L00317:246,
        F2021L00317:247,
        F2021L00317:248 ;
    dct:isPartOf F2021L00317:241 ;
    dct:isReferencedBy F2021L00317: ;
    rdfs:comment "Division 2 Functions and powers - Abrievated Graph Key: D244"@en-AU ;
    skos:broader F2021L00317:245,
        F2021L00317:246,
        F2021L00317:247,
        F2021L00317:248 ;
    skos:definition "Division 2 Functions and powers"@en-AU ;
    skos:narrower F2021L00317:241 ;
    skos:prefLabel "Division D244"@en-AU ;
    dcat:accessURL <https://www.legislation.gov.au/F2021L00317/asmade/2021-03-24/text/original/epub/OEBPS/document_1/document_1.html#_Toc66195001> ;
    dcat:landingPage "https://www.legislation.gov.au/F2021L00317/asmade/2021-03-24/text/original/epub/OEBPS/document_1/document_1.html#_Toc66195001"^^xsd:anyURI ;
    dcat:theme legcons:Division .

F2021L00317:256 a legcons:Chapter,
        owl:Class,
        dcat:Resource ;
    rdfs:label "Chapter - C256 Chapter 11 Miscellaneous"@en-AU ;
    dct:hasPart F2021L00317:257,
        F2021L00317:259,
        F2021L00317:269,
        F2021L00317:272,
        F2021L00317:275 ;
    dct:isReferencedBy F2021L00317: ;
    rdfs:comment "Chapter 11 Miscellaneous - Abrievated Graph Key: C256"@en-AU ;
    skos:broader F2021L00317:257,
        F2021L00317:259,
        F2021L00317:269,
        F2021L00317:272,
        F2021L00317:275 ;
    skos:definition "Chapter 11 Miscellaneous"@en-AU ;
    skos:prefLabel "Chapter C256"@en-AU ;
    dcat:accessURL <https://www.legislation.gov.au/F2021L00317/asmade/2021-03-24/text/original/epub/OEBPS/document_1/document_1.html#_Toc66195013> ;
    dcat:landingPage "https://www.legislation.gov.au/F2021L00317/asmade/2021-03-24/text/original/epub/OEBPS/document_1/document_1.html#_Toc66195013"^^xsd:anyURI ;
    dcat:theme legcons:Chapter .

F2021L00317:35 a legcons:Chapter,
        owl:Class,
        dcat:Resource ;
    rdfs:label "Chapter - C35 Chapter 4 Registered establishments"@en-AU ;
    dct:hasPart F2021L00317:36,
        F2021L00317:51,
        F2021L00317:55,
        F2021L00317:58,
        F2021L00317:61 ;
    dct:isReferencedBy F2021L00317: ;
    rdfs:comment "Chapter 4 Registered establishments - Abrievated Graph Key: C35"@en-AU ;
    skos:broader F2021L00317:36,
        F2021L00317:51,
        F2021L00317:55,
        F2021L00317:58,
        F2021L00317:61 ;
    skos:definition "Chapter 4 Registered establishments"@en-AU ;
    skos:prefLabel "Chapter C35"@en-AU ;
    dcat:accessURL <https://www.legislation.gov.au/F2021L00317/asmade/2021-03-24/text/original/epub/OEBPS/document_1/document_1.html#_Toc66194792> ;
    dcat:landingPage "https://www.legislation.gov.au/F2021L00317/asmade/2021-03-24/text/original/epub/OEBPS/document_1/document_1.html#_Toc66194792"^^xsd:anyURI ;
    dcat:theme legcons:Chapter .

F2021L00317:79 a legcons:Subdivision,
        owl:Class,
        dcat:Resource ;
    rdfs:label "Subdivision - S79 Subdivision APrescribed fish and fish productsgeneral"@en-AU ;
    dct:hasPart F2021L00317:80,
        F2021L00317:81,
        F2021L00317:82,
        F2021L00317:83 ;
    dct:isPartOf F2021L00317:77 ;
    dct:isReferencedBy F2021L00317: ;
    rdfs:comment "Subdivision APrescribed fish and fish productsgeneral - Abrievated Graph Key: S79"@en-AU ;
    skos:broader F2021L00317:80,
        F2021L00317:81,
        F2021L00317:82,
        F2021L00317:83 ;
    skos:definition "Subdivision APrescribed fish and fish productsgeneral"@en-AU ;
    skos:narrower F2021L00317:77 ;
    skos:prefLabel "Subdivision S79"@en-AU ;
    dcat:accessURL <https://www.legislation.gov.au/F2021L00317/asmade/2021-03-24/text/original/epub/OEBPS/document_1/document_1.html#_Toc66194836> ;
    dcat:landingPage "https://www.legislation.gov.au/F2021L00317/asmade/2021-03-24/text/original/epub/OEBPS/document_1/document_1.html#_Toc66194836"^^xsd:anyURI ;
    dcat:theme legcons:Subdivision .

F2021L00317:66 a legcons:Part,
        owl:Class,
        dcat:Resource ;
    rdfs:label "Part - P66 Part 1 Requirements for approval"@en-AU ;
    dct:hasPart F2021L00317:67,
        F2021L00317:68,
        F2021L00317:69,
        F2021L00317:70,
        F2021L00317:71 ;
    dct:isPartOf F2021L00317:65 ;
    dct:isReferencedBy F2021L00317: ;
    rdfs:comment "Part 1 Requirements for approval - Abrievated Graph Key: P66"@en-AU ;
    skos:broader F2021L00317:67,
        F2021L00317:68,
        F2021L00317:69,
        F2021L00317:70,
        F2021L00317:71 ;
    skos:definition "Part 1 Requirements for approval"@en-AU ;
    skos:narrower F2021L00317:65 ;
    skos:prefLabel "Part P66"@en-AU ;
    dcat:accessURL <https://www.legislation.gov.au/F2021L00317/asmade/2021-03-24/text/original/epub/OEBPS/document_1/document_1.html#_Toc66194823> ;
    dcat:landingPage "https://www.legislation.gov.au/F2021L00317/asmade/2021-03-24/text/original/epub/OEBPS/document_1/document_1.html#_Toc66194823"^^xsd:anyURI ;
    dcat:theme legcons:Part .

F2021L00317:77 a legcons:Division,
        owl:Class,
        dcat:Resource ;
    rdfs:label "Division - D77 Division 3 Operational hygiene"@en-AU ;
    dct:hasPart F2021L00317:78,
        F2021L00317:79,
        F2021L00317:84,
        F2021L00317:85,
        F2021L00317:86 ;
    dct:isPartOf F2021L00317:72 ;
    dct:isReferencedBy F2021L00317: ;
    rdfs:comment "Division 3 Operational hygiene - Abrievated Graph Key: D77"@en-AU ;
    skos:broader F2021L00317:78,
        F2021L00317:79,
        F2021L00317:84,
        F2021L00317:85,
        F2021L00317:86 ;
    skos:definition "Division 3 Operational hygiene"@en-AU ;
    skos:narrower F2021L00317:72 ;
    skos:prefLabel "Division D77"@en-AU ;
    dcat:accessURL <https://www.legislation.gov.au/F2021L00317/asmade/2021-03-24/text/original/epub/OEBPS/document_1/document_1.html#_Toc66194834> ;
    dcat:landingPage "https://www.legislation.gov.au/F2021L00317/asmade/2021-03-24/text/original/epub/OEBPS/document_1/document_1.html#_Toc66194834"^^xsd:anyURI ;
    dcat:theme legcons:Division .

F2021L00317:192 a legcons:Division,
        owl:Class,
        dcat:Resource ;
    rdfs:label "Division - D192 Division 4 Official marking devices"@en-AU ;
    dct:hasPart F2021L00317:193,
        F2021L00317:194,
        F2021L00317:195,
        F2021L00317:196,
        F2021L00317:197,
        F2021L00317:198 ;
    dct:isPartOf F2021L00317:164 ;
    dct:isReferencedBy F2021L00317: ;
    rdfs:comment "Division 4 Official marking devices - Abrievated Graph Key: D192"@en-AU ;
    skos:broader F2021L00317:193,
        F2021L00317:194,
        F2021L00317:195,
        F2021L00317:196,
        F2021L00317:197,
        F2021L00317:198 ;
    skos:definition "Division 4 Official marking devices"@en-AU ;
    skos:narrower F2021L00317:164 ;
    skos:prefLabel "Division D192"@en-AU ;
    dcat:accessURL <https://www.legislation.gov.au/F2021L00317/asmade/2021-03-24/text/original/epub/OEBPS/document_1/document_1.html#_Toc66194949> ;
    dcat:landingPage "https://www.legislation.gov.au/F2021L00317/asmade/2021-03-24/text/original/epub/OEBPS/document_1/document_1.html#_Toc66194949"^^xsd:anyURI ;
    dcat:theme legcons:Division .

F2021L00317:1 a legcons:Chapter,
        owl:Class,
        dcat:Resource ;
    rdfs:label "Chapter - C1 Chapter 1 Preliminary"@en-AU ;
    dct:hasPart F2021L00317:10,
        F2021L00317:2,
        F2021L00317:3,
        F2021L00317:4,
        F2021L00317:5,
        F2021L00317:6,
        F2021L00317:7,
        F2021L00317:8,
        F2021L00317:9 ;
    dct:isReferencedBy F2021L00317: ;
    rdfs:comment "Chapter 1 Preliminary - Abrievated Graph Key: C1"@en-AU ;
    skos:broader F2021L00317:10,
        F2021L00317:2,
        F2021L00317:3,
        F2021L00317:4,
        F2021L00317:5,
        F2021L00317:6,
        F2021L00317:7,
        F2021L00317:8,
        F2021L00317:9 ;
    skos:definition "Chapter 1 Preliminary"@en-AU ;
    skos:prefLabel "Chapter C1"@en-AU ;
    dcat:accessURL <https://www.legislation.gov.au/F2021L00317/asmade/2021-03-24/text/original/epub/OEBPS/document_1/document_1.html#_Toc66194758> ;
    dcat:landingPage "https://www.legislation.gov.au/F2021L00317/asmade/2021-03-24/text/original/epub/OEBPS/document_1/document_1.html#_Toc66194758"^^xsd:anyURI ;
    dcat:theme legcons:Chapter .

F2021L00317:165 a legcons:Division,
        owl:Class,
        dcat:Resource ;
    rdfs:label "Division - D165 Division 1 Marks that are official marks"@en-AU ;
    dct:hasPart F2021L00317:166,
        F2021L00317:167,
        F2021L00317:168,
        F2021L00317:169,
        F2021L00317:170,
        F2021L00317:171,
        F2021L00317:172,
        F2021L00317:173,
        F2021L00317:174 ;
    dct:isPartOf F2021L00317:164 ;
    dct:isReferencedBy F2021L00317: ;
    rdfs:comment "Division 1 Marks that are official marks - Abrievated Graph Key: D165"@en-AU ;
    skos:broader F2021L00317:166,
        F2021L00317:167,
        F2021L00317:168,
        F2021L00317:169,
        F2021L00317:170,
        F2021L00317:171,
        F2021L00317:172,
        F2021L00317:173,
        F2021L00317:174 ;
    skos:definition "Division 1 Marks that are official marks"@en-AU ;
    skos:narrower F2021L00317:164 ;
    skos:prefLabel "Division D165"@en-AU ;
    dcat:accessURL <https://www.legislation.gov.au/F2021L00317/asmade/2021-03-24/text/original/epub/OEBPS/document_1/document_1.html#_Toc66194922> ;
    dcat:landingPage "https://www.legislation.gov.au/F2021L00317/asmade/2021-03-24/text/original/epub/OEBPS/document_1/document_1.html#_Toc66194922"^^xsd:anyURI ;
    dcat:theme legcons:Division .

F2021L00317:259 a legcons:Part,
        owl:Class,
        dcat:Resource ;
    rdfs:label "Part - P259 Part 2 Records"@en-AU ;
    dct:hasPart F2021L00317:260,
        F2021L00317:261,
        F2021L00317:262,
        F2021L00317:263,
        F2021L00317:264,
        F2021L00317:265,
        F2021L00317:266,
        F2021L00317:267,
        F2021L00317:268 ;
    dct:isPartOf F2021L00317:256 ;
    dct:isReferencedBy F2021L00317: ;
    rdfs:comment "Part 2 Records - Abrievated Graph Key: P259"@en-AU ;
    skos:broader F2021L00317:260,
        F2021L00317:261,
        F2021L00317:262,
        F2021L00317:263,
        F2021L00317:264,
        F2021L00317:265,
        F2021L00317:266,
        F2021L00317:267,
        F2021L00317:268 ;
    skos:definition "Part 2 Records"@en-AU ;
    skos:narrower F2021L00317:256 ;
    skos:prefLabel "Part P259"@en-AU ;
    dcat:accessURL <https://www.legislation.gov.au/F2021L00317/asmade/2021-03-24/text/original/epub/OEBPS/document_1/document_1.html#_Toc66195016> ;
    dcat:landingPage "https://www.legislation.gov.au/F2021L00317/asmade/2021-03-24/text/original/epub/OEBPS/document_1/document_1.html#_Toc66195016"^^xsd:anyURI ;
    dcat:theme legcons:Part .

F2021L00317:37 a legcons:Division,
        owl:Class,
        dcat:Resource ;
    rdfs:label "Division - D37 Division 1 Requirements relating to construction equipment and facilities"@en-AU ;
    dct:hasPart F2021L00317:38,
        F2021L00317:39,
        F2021L00317:40,
        F2021L00317:41,
        F2021L00317:42,
        F2021L00317:43,
        F2021L00317:44,
        F2021L00317:45,
        F2021L00317:46,
        F2021L00317:47 ;
    dct:isPartOf F2021L00317:36 ;
    dct:isReferencedBy F2021L00317: ;
    rdfs:comment "Division 1 Requirements relating to construction equipment and facilities - Abrievated Graph Key: D37"@en-AU ;
    skos:broader F2021L00317:38,
        F2021L00317:39,
        F2021L00317:40,
        F2021L00317:41,
        F2021L00317:42,
        F2021L00317:43,
        F2021L00317:44,
        F2021L00317:45,
        F2021L00317:46,
        F2021L00317:47 ;
    skos:definition "Division 1 Requirements relating to construction equipment and facilities"@en-AU ;
    skos:narrower F2021L00317:36 ;
    skos:prefLabel "Division D37"@en-AU ;
    dcat:accessURL <https://www.legislation.gov.au/F2021L00317/asmade/2021-03-24/text/original/epub/OEBPS/document_1/document_1.html#_Toc66194794> ;
    dcat:landingPage "https://www.legislation.gov.au/F2021L00317/asmade/2021-03-24/text/original/epub/OEBPS/document_1/document_1.html#_Toc66194794"^^xsd:anyURI ;
    dcat:theme legcons:Division .

F2021L00317:65 a legcons:Chapter,
        owl:Class,
        dcat:Resource ;
    rdfs:label "Chapter - C65 Chapter 5 Approved arrangements"@en-AU ;
    dct:hasPart F2021L00317:132,
        F2021L00317:133,
        F2021L00317:134,
        F2021L00317:135,
        F2021L00317:138,
        F2021L00317:140,
        F2021L00317:141,
        F2021L00317:142,
        F2021L00317:143,
        F2021L00317:66,
        F2021L00317:72 ;
    dct:isReferencedBy F2021L00317: ;
    rdfs:comment "Chapter 5 Approved arrangements - Abrievated Graph Key: C65"@en-AU ;
    skos:broader F2021L00317:132,
        F2021L00317:133,
        F2021L00317:134,
        F2021L00317:135,
        F2021L00317:138,
        F2021L00317:140,
        F2021L00317:141,
        F2021L00317:142,
        F2021L00317:143,
        F2021L00317:66,
        F2021L00317:72 ;
    skos:definition "Chapter 5 Approved arrangements"@en-AU ;
    skos:prefLabel "Chapter C65"@en-AU ;
    dcat:accessURL <https://www.legislation.gov.au/F2021L00317/asmade/2021-03-24/text/original/epub/OEBPS/document_1/document_1.html#_Toc66194822> ;
    dcat:landingPage "https://www.legislation.gov.au/F2021L00317/asmade/2021-03-24/text/original/epub/OEBPS/document_1/document_1.html#_Toc66194822"^^xsd:anyURI ;
    dcat:theme legcons:Chapter .

F2021L00317:209 a legcons:Division,
        owl:Class,
        dcat:Resource ;
    rdfs:label "Division - D209 Division 3 Approved auditors"@en-AU ;
    dct:hasPart F2021L00317:210,
        F2021L00317:211,
        F2021L00317:212,
        F2021L00317:213,
        F2021L00317:214,
        F2021L00317:215,
        F2021L00317:216,
        F2021L00317:217,
        F2021L00317:218,
        F2021L00317:219,
        F2021L00317:220 ;
    dct:isPartOf F2021L00317:200 ;
    dct:isReferencedBy F2021L00317: ;
    rdfs:comment "Division 3 Approved auditors - Abrievated Graph Key: D209"@en-AU ;
    skos:broader F2021L00317:210,
        F2021L00317:211,
        F2021L00317:212,
        F2021L00317:213,
        F2021L00317:214,
        F2021L00317:215,
        F2021L00317:216,
        F2021L00317:217,
        F2021L00317:218,
        F2021L00317:219,
        F2021L00317:220 ;
    skos:definition "Division 3 Approved auditors"@en-AU ;
    skos:narrower F2021L00317:200 ;
    skos:prefLabel "Division D209"@en-AU ;
    dcat:accessURL <https://www.legislation.gov.au/F2021L00317/asmade/2021-03-24/text/original/epub/OEBPS/document_1/document_1.html#_Toc66194966> ;
    dcat:landingPage "https://www.legislation.gov.au/F2021L00317/asmade/2021-03-24/text/original/epub/OEBPS/document_1/document_1.html#_Toc66194966"^^xsd:anyURI ;
    dcat:theme legcons:Division .

F2021L00317:227 a legcons:Division,
        owl:Class,
        dcat:Resource ;
    rdfs:label "Division - D227 Division 3 Approved assessors"@en-AU ;
    dct:hasPart F2021L00317:228,
        F2021L00317:229,
        F2021L00317:230,
        F2021L00317:231,
        F2021L00317:232,
        F2021L00317:233,
        F2021L00317:234,
        F2021L00317:235,
        F2021L00317:236,
        F2021L00317:237,
        F2021L00317:238 ;
    dct:isPartOf F2021L00317:221 ;
    dct:isReferencedBy F2021L00317: ;
    rdfs:comment "Division 3 Approved assessors - Abrievated Graph Key: D227"@en-AU ;
    skos:broader F2021L00317:228,
        F2021L00317:229,
        F2021L00317:230,
        F2021L00317:231,
        F2021L00317:232,
        F2021L00317:233,
        F2021L00317:234,
        F2021L00317:235,
        F2021L00317:236,
        F2021L00317:237,
        F2021L00317:238 ;
    skos:definition "Division 3 Approved assessors"@en-AU ;
    skos:narrower F2021L00317:221 ;
    skos:prefLabel "Division D227"@en-AU ;
    dcat:accessURL <https://www.legislation.gov.au/F2021L00317/asmade/2021-03-24/text/original/epub/OEBPS/document_1/document_1.html#_Toc66194984> ;
    dcat:landingPage "https://www.legislation.gov.au/F2021L00317/asmade/2021-03-24/text/original/epub/OEBPS/document_1/document_1.html#_Toc66194984"^^xsd:anyURI ;
    dcat:theme legcons:Division .

F2021L00317:175 a legcons:Division,
        owl:Class,
        dcat:Resource ;
    rdfs:label "Division - D175 Division 2 General rules relating to official marks"@en-AU ;
    dct:hasPart F2021L00317:176,
        F2021L00317:177,
        F2021L00317:178,
        F2021L00317:179,
        F2021L00317:180,
        F2021L00317:181,
        F2021L00317:182,
        F2021L00317:183,
        F2021L00317:184,
        F2021L00317:185,
        F2021L00317:186,
        F2021L00317:187 ;
    dct:isPartOf F2021L00317:164 ;
    dct:isReferencedBy F2021L00317: ;
    rdfs:comment "Division 2 General rules relating to official marks - Abrievated Graph Key: D175"@en-AU ;
    skos:broader F2021L00317:176,
        F2021L00317:177,
        F2021L00317:178,
        F2021L00317:179,
        F2021L00317:180,
        F2021L00317:181,
        F2021L00317:182,
        F2021L00317:183,
        F2021L00317:184,
        F2021L00317:185,
        F2021L00317:186,
        F2021L00317:187 ;
    skos:definition "Division 2 General rules relating to official marks"@en-AU ;
    skos:narrower F2021L00317:164 ;
    skos:prefLabel "Division D175"@en-AU ;
    dcat:accessURL <https://www.legislation.gov.au/F2021L00317/asmade/2021-03-24/text/original/epub/OEBPS/document_1/document_1.html#_Toc66194932> ;
    dcat:landingPage "https://www.legislation.gov.au/F2021L00317/asmade/2021-03-24/text/original/epub/OEBPS/document_1/document_1.html#_Toc66194932"^^xsd:anyURI ;
    dcat:theme legcons:Division .

F2021L00317:88 a legcons:Subdivision,
        owl:Class,
        dcat:Resource ;
    rdfs:label "Subdivision - S88 Subdivision APrescribed fish and fish productsgeneral"@en-AU ;
    dct:hasPart F2021L00317:100,
        F2021L00317:101,
        F2021L00317:102,
        F2021L00317:89,
        F2021L00317:90,
        F2021L00317:91,
        F2021L00317:92,
        F2021L00317:93,
        F2021L00317:94,
        F2021L00317:95,
        F2021L00317:96,
        F2021L00317:97,
        F2021L00317:98,
        F2021L00317:99 ;
    dct:isPartOf F2021L00317:72 ;
    dct:isReferencedBy F2021L00317: ;
    rdfs:comment "Subdivision APrescribed fish and fish productsgeneral - Abrievated Graph Key: S88"@en-AU ;
    skos:broader F2021L00317:100,
        F2021L00317:101,
        F2021L00317:102,
        F2021L00317:89,
        F2021L00317:90,
        F2021L00317:91,
        F2021L00317:92,
        F2021L00317:93,
        F2021L00317:94,
        F2021L00317:95,
        F2021L00317:96,
        F2021L00317:97,
        F2021L00317:98,
        F2021L00317:99 ;
    skos:definition "Subdivision APrescribed fish and fish productsgeneral"@en-AU ;
    skos:narrower F2021L00317:72 ;
    skos:prefLabel "Subdivision S88"@en-AU ;
    dcat:accessURL <https://www.legislation.gov.au/F2021L00317/asmade/2021-03-24/text/original/epub/OEBPS/document_1/document_1.html#_Toc66194845> ;
    dcat:landingPage "https://www.legislation.gov.au/F2021L00317/asmade/2021-03-24/text/original/epub/OEBPS/document_1/document_1.html#_Toc66194845"^^xsd:anyURI ;
    dcat:theme legcons:Subdivision .

F2021L00317:11 a legcons:Chapter,
        owl:Class,
        dcat:Resource ;
    rdfs:label "Chapter - C11 Chapter 2 Exporting goods"@en-AU ;
    dct:hasPart F2021L00317:12,
        F2021L00317:19,
        F2021L00317:20,
        F2021L00317:21,
        F2021L00317:22,
        F2021L00317:23,
        F2021L00317:24,
        F2021L00317:25,
        F2021L00317:26,
        F2021L00317:27,
        F2021L00317:28,
        F2021L00317:29,
        F2021L00317:30,
        F2021L00317:31,
        F2021L00317:32,
        F2021L00317:33,
        F2021L00317:34 ;
    dct:isReferencedBy F2021L00317: ;
    rdfs:comment "Chapter 2 Exporting goods - Abrievated Graph Key: C11"@en-AU ;
    skos:broader F2021L00317:12,
        F2021L00317:19,
        F2021L00317:20,
        F2021L00317:21,
        F2021L00317:22,
        F2021L00317:23,
        F2021L00317:24,
        F2021L00317:25,
        F2021L00317:26,
        F2021L00317:27,
        F2021L00317:28,
        F2021L00317:29,
        F2021L00317:30,
        F2021L00317:31,
        F2021L00317:32,
        F2021L00317:33,
        F2021L00317:34 ;
    skos:definition "Chapter 2 Exporting goods"@en-AU ;
    skos:prefLabel "Chapter C11"@en-AU ;
    dcat:accessURL <https://www.legislation.gov.au/F2021L00317/asmade/2021-03-24/text/original/epub/OEBPS/document_1/document_1.html#_Toc66194768> ;
    dcat:landingPage "https://www.legislation.gov.au/F2021L00317/asmade/2021-03-24/text/original/epub/OEBPS/document_1/document_1.html#_Toc66194768"^^xsd:anyURI ;
    dcat:theme legcons:Chapter .

F2021L00317:72 a legcons:Part,
        owl:Class,
        dcat:Resource ;
    rdfs:label "Part - P72 Part 2 Conditions of approved arrangement"@en-AU ;
    dct:hasPart F2021L00317:103,
        F2021L00317:107,
        F2021L00317:111,
        F2021L00317:112,
        F2021L00317:113,
        F2021L00317:114,
        F2021L00317:115,
        F2021L00317:116,
        F2021L00317:117,
        F2021L00317:118,
        F2021L00317:119,
        F2021L00317:120,
        F2021L00317:121,
        F2021L00317:122,
        F2021L00317:123,
        F2021L00317:124,
        F2021L00317:125,
        F2021L00317:126,
        F2021L00317:127,
        F2021L00317:128,
        F2021L00317:129,
        F2021L00317:130,
        F2021L00317:131,
        F2021L00317:73,
        F2021L00317:75,
        F2021L00317:77,
        F2021L00317:87,
        F2021L00317:88 ;
    dct:isPartOf F2021L00317:65 ;
    dct:isReferencedBy F2021L00317: ;
    rdfs:comment "Part 2 Conditions of approved arrangement - Abrievated Graph Key: P72"@en-AU ;
    skos:broader F2021L00317:103,
        F2021L00317:107,
        F2021L00317:111,
        F2021L00317:112,
        F2021L00317:113,
        F2021L00317:114,
        F2021L00317:115,
        F2021L00317:116,
        F2021L00317:117,
        F2021L00317:118,
        F2021L00317:119,
        F2021L00317:120,
        F2021L00317:121,
        F2021L00317:122,
        F2021L00317:123,
        F2021L00317:124,
        F2021L00317:125,
        F2021L00317:126,
        F2021L00317:127,
        F2021L00317:128,
        F2021L00317:129,
        F2021L00317:130,
        F2021L00317:131,
        F2021L00317:73,
        F2021L00317:75,
        F2021L00317:77,
        F2021L00317:87,
        F2021L00317:88 ;
    skos:definition "Part 2 Conditions of approved arrangement"@en-AU ;
    skos:narrower F2021L00317:65 ;
    skos:prefLabel "Part P72"@en-AU ;
    dcat:accessURL <https://www.legislation.gov.au/F2021L00317/asmade/2021-03-24/text/original/epub/OEBPS/document_1/document_1.html#_Toc66194829> ;
    dcat:landingPage "https://www.legislation.gov.au/F2021L00317/asmade/2021-03-24/text/original/epub/OEBPS/document_1/document_1.html#_Toc66194829"^^xsd:anyURI ;
    dcat:theme legcons:Part .

F2021L00317: a owl:Class,
        dcat:Dataset,
        dcat:Resource ;
    rdfs:label "Export Control (Fish and Fish Products) Rules 2021" ;
    dct:Jurisdiction " Department of Agriculture, Fisheries and Forestry "@en-AU ;
    dct:created "2024-08-30T15:13:36.223392"^^xsd:dateTime ;
    dct:creator "https://orcid.org/0009-0007-8434-7325"^^xsd:anyURI ;
    dct:date "2021-03-24T00:00:00+11:00"^^xsd:dateTime ;
    dct:description "Export Control (Fish and Fish Products) Rules 2021"@en-AU ;
    dct:identifier "https://www.legislation.gov.au/F2021L00317/asmade"^^xsd:anyURI ;
    dct:license <https://creativecommons.org/licenses/by-sa/4.0/> ;
    dct:source "scheme=AGLSTERMS.AglsAgent; corporateName=Office Parliamentary Counsel; address=Locked Bag 30 Kingston ACT 2604; contact=+61 2 6120 1400"@en-AU ;
    dct:subject "Export Control (Fish and Fish Products) Rules 2021"@en-AU ;
    dct:title "Export Control (Fish and Fish Products) Rules 2021"@en-AU ;
    owl:imports legcons: ;
    dcat:theme legcons:Chapter,
        legcons:Division,
        legcons:Item,
        legcons:Part,
        legcons:Subdivision ;
    schema:identifier "F2021L00317" ;
    schema:status "In force" ;
    schema:version "F2021L00317" .

