@prefix F2021L00319: <http://example.org/au/leg/dataset/F2021L00319/> .
@prefix dcat: <http://www.w3.org/ns/dcat#> .
@prefix dct: <http://purl.org/dc/terms/> .
@prefix legcons: <http://example.org/au/leg/concepts/> .
@prefix owl: <http://www.w3.org/2002/07/owl#> .
@prefix rdfs: <http://www.w3.org/2000/01/rdf-schema#> .
@prefix schema: <https://schema.org/> .
@prefix skos: <http://www.w3.org/2004/02/skos/core#> .
@prefix xsd: <http://www.w3.org/2001/XMLSchema#> .

F2021L00319:100 a legcons:Item,
        owl:Class,
        dcat:Resource ;
    rdfs:label "Item - I100 5 14  Purpose of this Division"@en-AU ;
    dct:isPartOf F2021L00319:99 ;
    dct:isReferencedBy F2021L00319: ;
    rdfs:comment "5 14  Purpose of this Division - Abrievated Graph Key: I100"@en-AU ;
    skos:definition "5 14  Purpose of this Division"@en-AU ;
    skos:narrower F2021L00319:99 ;
    skos:prefLabel "Item I100"@en-AU ;
    dcat:accessURL <https://www.legislation.gov.au/F2021L00319/2024-04-30/2024-04-30/text/original/epub/OEBPS/document_1/document_1.html#_Toc166157933> ;
    dcat:landingPage "https://www.legislation.gov.au/F2021L00319/2024-04-30/2024-04-30/text/original/epub/OEBPS/document_1/document_1.html#_Toc166157933"^^xsd:anyURI ;
    dcat:theme legcons:Item .

F2021L00319:101 a legcons:Item,
        owl:Class,
        dcat:Resource ;
    rdfs:label "Item - I101 5 15  Requirements for approval must continue to be met"@en-AU ;
    dct:isPartOf F2021L00319:99 ;
    dct:isReferencedBy F2021L00319: ;
    rdfs:comment "5 15  Requirements for approval must continue to be met - Abrievated Graph Key: I101"@en-AU ;
    skos:definition "5 15  Requirements for approval must continue to be met"@en-AU ;
    skos:narrower F2021L00319:99 ;
    skos:prefLabel "Item I101"@en-AU ;
    dcat:accessURL <https://www.legislation.gov.au/F2021L00319/2024-04-30/2024-04-30/text/original/epub/OEBPS/document_1/document_1.html#_Toc166157934> ;
    dcat:landingPage "https://www.legislation.gov.au/F2021L00319/2024-04-30/2024-04-30/text/original/epub/OEBPS/document_1/document_1.html#_Toc166157934"^^xsd:anyURI ;
    dcat:theme legcons:Item .

F2021L00319:102 a legcons:Item,
        owl:Class,
        dcat:Resource ;
    rdfs:label "Item - I102 5 16  Compliance with assurance rules and meeting assurance standards"@en-AU ;
    dct:isPartOf F2021L00319:99 ;
    dct:isReferencedBy F2021L00319: ;
    rdfs:comment "5 16  Compliance with assurance rules and meeting assurance standards - Abrievated Graph Key: I102"@en-AU ;
    skos:definition "5 16  Compliance with assurance rules and meeting assurance standards"@en-AU ;
    skos:narrower F2021L00319:99 ;
    skos:prefLabel "Item I102"@en-AU ;
    dcat:accessURL <https://www.legislation.gov.au/F2021L00319/2024-04-30/2024-04-30/text/original/epub/OEBPS/document_1/document_1.html#_Toc166157935> ;
    dcat:landingPage "https://www.legislation.gov.au/F2021L00319/2024-04-30/2024-04-30/text/original/epub/OEBPS/document_1/document_1.html#_Toc166157935"^^xsd:anyURI ;
    dcat:theme legcons:Item .

F2021L00319:103 a legcons:Item,
        owl:Class,
        dcat:Resource ;
    rdfs:label "Item - I103 5 17  Information must be given to the Secretary about entities in relation to which exporter supply chain assurance operations have been carried out"@en-AU ;
    dct:isPartOf F2021L00319:99 ;
    dct:isReferencedBy F2021L00319: ;
    rdfs:comment "5 17  Information must be given to the Secretary about entities in relation to which exporter supply chain assurance operations have been carried out - Abrievated Graph Key: I103"@en-AU ;
    skos:definition "5 17  Information must be given to the Secretary about entities in relation to which exporter supply chain assurance operations have been carried out"@en-AU ;
    skos:narrower F2021L00319:99 ;
    skos:prefLabel "Item I103"@en-AU ;
    dcat:accessURL <https://www.legislation.gov.au/F2021L00319/2024-04-30/2024-04-30/text/original/epub/OEBPS/document_1/document_1.html#_Toc166157936> ;
    dcat:landingPage "https://www.legislation.gov.au/F2021L00319/2024-04-30/2024-04-30/text/original/epub/OEBPS/document_1/document_1.html#_Toc166157936"^^xsd:anyURI ;
    dcat:theme legcons:Item .

F2021L00319:104 a legcons:Item,
        owl:Class,
        dcat:Resource ;
    rdfs:label "Item - I104 5 18  Report to Secretary on exporter supply chain assurance operations carried out"@en-AU ;
    dct:isPartOf F2021L00319:99 ;
    dct:isReferencedBy F2021L00319: ;
    rdfs:comment "5 18  Report to Secretary on exporter supply chain assurance operations carried out - Abrievated Graph Key: I104"@en-AU ;
    skos:definition "5 18  Report to Secretary on exporter supply chain assurance operations carried out"@en-AU ;
    skos:narrower F2021L00319:99 ;
    skos:prefLabel "Item I104"@en-AU ;
    dcat:accessURL <https://www.legislation.gov.au/F2021L00319/2024-04-30/2024-04-30/text/original/epub/OEBPS/document_1/document_1.html#_Toc166157937> ;
    dcat:landingPage "https://www.legislation.gov.au/F2021L00319/2024-04-30/2024-04-30/text/original/epub/OEBPS/document_1/document_1.html#_Toc166157937"^^xsd:anyURI ;
    dcat:theme legcons:Item .

F2021L00319:106 a legcons:Item,
        owl:Class,
        dcat:Resource ;
    rdfs:label "Item - I106 5 19  Period within which application to renew approved arrangement must be made"@en-AU ;
    dct:isPartOf F2021L00319:105 ;
    dct:isReferencedBy F2021L00319: ;
    rdfs:comment "5 19  Period within which application to renew approved arrangement must be made - Abrievated Graph Key: I106"@en-AU ;
    skos:definition "5 19  Period within which application to renew approved arrangement must be made"@en-AU ;
    skos:narrower F2021L00319:105 ;
    skos:prefLabel "Item I106"@en-AU ;
    dcat:accessURL <https://www.legislation.gov.au/F2021L00319/2024-04-30/2024-04-30/text/original/epub/OEBPS/document_1/document_1.html#_Toc166157939> ;
    dcat:landingPage "https://www.legislation.gov.au/F2021L00319/2024-04-30/2024-04-30/text/original/epub/OEBPS/document_1/document_1.html#_Toc166157939"^^xsd:anyURI ;
    dcat:theme legcons:Item .

F2021L00319:108 a legcons:Item,
        owl:Class,
        dcat:Resource ;
    rdfs:label "Item - I108 5 20  Application by holder for variationgrounds for refusing application"@en-AU ;
    dct:isPartOf F2021L00319:107 ;
    dct:isReferencedBy F2021L00319: ;
    rdfs:comment "5 20  Application by holder for variationgrounds for refusing application - Abrievated Graph Key: I108"@en-AU ;
    skos:definition "5 20  Application by holder for variationgrounds for refusing application"@en-AU ;
    skos:narrower F2021L00319:107 ;
    skos:prefLabel "Item I108"@en-AU ;
    dcat:accessURL <https://www.legislation.gov.au/F2021L00319/2024-04-30/2024-04-30/text/original/epub/OEBPS/document_1/document_1.html#_Toc166157941> ;
    dcat:landingPage "https://www.legislation.gov.au/F2021L00319/2024-04-30/2024-04-30/text/original/epub/OEBPS/document_1/document_1.html#_Toc166157941"^^xsd:anyURI ;
    dcat:theme legcons:Item .

F2021L00319:109 a legcons:Item,
        owl:Class,
        dcat:Resource ;
    rdfs:label "Item - I109 5 21  Significant variations"@en-AU ;
    dct:isPartOf F2021L00319:107 ;
    dct:isReferencedBy F2021L00319: ;
    rdfs:comment "5 21  Significant variations - Abrievated Graph Key: I109"@en-AU ;
    skos:definition "5 21  Significant variations"@en-AU ;
    skos:narrower F2021L00319:107 ;
    skos:prefLabel "Item I109"@en-AU ;
    dcat:accessURL <https://www.legislation.gov.au/F2021L00319/2024-04-30/2024-04-30/text/original/epub/OEBPS/document_1/document_1.html#_Toc166157942> ;
    dcat:landingPage "https://www.legislation.gov.au/F2021L00319/2024-04-30/2024-04-30/text/original/epub/OEBPS/document_1/document_1.html#_Toc166157942"^^xsd:anyURI ;
    dcat:theme legcons:Item .

F2021L00319:111 a legcons:Item,
        owl:Class,
        dcat:Resource ;
    rdfs:label "Item - I111 5 21 A  Suspension requested by holderprescribed circumstances"@en-AU ;
    dct:isPartOf F2021L00319:110 ;
    dct:isReferencedBy F2021L00319: ;
    rdfs:comment "5 21 A  Suspension requested by holderprescribed circumstances - Abrievated Graph Key: I111"@en-AU ;
    skos:definition "5 21 A  Suspension requested by holderprescribed circumstances"@en-AU ;
    skos:narrower F2021L00319:110 ;
    skos:prefLabel "Item I111"@en-AU ;
    dcat:accessURL <https://www.legislation.gov.au/F2021L00319/2024-04-30/2024-04-30/text/original/epub/OEBPS/document_1/document_1.html#_Toc166157944> ;
    dcat:landingPage "https://www.legislation.gov.au/F2021L00319/2024-04-30/2024-04-30/text/original/epub/OEBPS/document_1/document_1.html#_Toc166157944"^^xsd:anyURI ;
    dcat:theme legcons:Item .

F2021L00319:112 a legcons:Item,
        owl:Class,
        dcat:Resource ;
    rdfs:label "Item - I112 5 21 B  Suspension requested by holderprescribed information"@en-AU ;
    dct:isPartOf F2021L00319:110 ;
    dct:isReferencedBy F2021L00319: ;
    rdfs:comment "5 21 B  Suspension requested by holderprescribed information - Abrievated Graph Key: I112"@en-AU ;
    skos:definition "5 21 B  Suspension requested by holderprescribed information"@en-AU ;
    skos:narrower F2021L00319:110 ;
    skos:prefLabel "Item I112"@en-AU ;
    dcat:accessURL <https://www.legislation.gov.au/F2021L00319/2024-04-30/2024-04-30/text/original/epub/OEBPS/document_1/document_1.html#_Toc166157945> ;
    dcat:landingPage "https://www.legislation.gov.au/F2021L00319/2024-04-30/2024-04-30/text/original/epub/OEBPS/document_1/document_1.html#_Toc166157945"^^xsd:anyURI ;
    dcat:theme legcons:Item .

F2021L00319:113 a legcons:Item,
        owl:Class,
        dcat:Resource ;
    rdfs:label "Item - I113 5 22  Suspension by Secretaryother grounds for suspension"@en-AU ;
    dct:isPartOf F2021L00319:110 ;
    dct:isReferencedBy F2021L00319: ;
    rdfs:comment "5 22  Suspension by Secretaryother grounds for suspension - Abrievated Graph Key: I113"@en-AU ;
    skos:definition "5 22  Suspension by Secretaryother grounds for suspension"@en-AU ;
    skos:narrower F2021L00319:110 ;
    skos:prefLabel "Item I113"@en-AU ;
    dcat:accessURL <https://www.legislation.gov.au/F2021L00319/2024-04-30/2024-04-30/text/original/epub/OEBPS/document_1/document_1.html#_Toc166157946> ;
    dcat:landingPage "https://www.legislation.gov.au/F2021L00319/2024-04-30/2024-04-30/text/original/epub/OEBPS/document_1/document_1.html#_Toc166157946"^^xsd:anyURI ;
    dcat:theme legcons:Item .

F2021L00319:115 a legcons:Item,
        owl:Class,
        dcat:Resource ;
    rdfs:label "Item - I115 5 23  Other grounds for revocation"@en-AU ;
    dct:isPartOf F2021L00319:114 ;
    dct:isReferencedBy F2021L00319: ;
    rdfs:comment "5 23  Other grounds for revocation - Abrievated Graph Key: I115"@en-AU ;
    skos:definition "5 23  Other grounds for revocation"@en-AU ;
    skos:narrower F2021L00319:114 ;
    skos:prefLabel "Item I115"@en-AU ;
    dcat:accessURL <https://www.legislation.gov.au/F2021L00319/2024-04-30/2024-04-30/text/original/epub/OEBPS/document_1/document_1.html#_Toc166157948> ;
    dcat:landingPage "https://www.legislation.gov.au/F2021L00319/2024-04-30/2024-04-30/text/original/epub/OEBPS/document_1/document_1.html#_Toc166157948"^^xsd:anyURI ;
    dcat:theme legcons:Item .

F2021L00319:117 a legcons:Item,
        owl:Class,
        dcat:Resource ;
    rdfs:label "Item - I117 5 24  Kinds of persons who are required to be fit and proper persons"@en-AU ;
    dct:isPartOf F2021L00319:116 ;
    dct:isReferencedBy F2021L00319: ;
    rdfs:comment "5 24  Kinds of persons who are required to be fit and proper persons - Abrievated Graph Key: I117"@en-AU ;
    skos:definition "5 24  Kinds of persons who are required to be fit and proper persons"@en-AU ;
    skos:narrower F2021L00319:116 ;
    skos:prefLabel "Item I117"@en-AU ;
    dcat:accessURL <https://www.legislation.gov.au/F2021L00319/2024-04-30/2024-04-30/text/original/epub/OEBPS/document_1/document_1.html#_Toc166157950> ;
    dcat:landingPage "https://www.legislation.gov.au/F2021L00319/2024-04-30/2024-04-30/text/original/epub/OEBPS/document_1/document_1.html#_Toc166157950"^^xsd:anyURI ;
    dcat:theme legcons:Item .

F2021L00319:119 a legcons:Item,
        owl:Class,
        dcat:Resource ;
    rdfs:label "Item - I119 5 25  Secretary may publish information given by holder of approved arrangement for exporter supply chain assurance operations"@en-AU ;
    dct:isPartOf F2021L00319:118 ;
    dct:isReferencedBy F2021L00319: ;
    rdfs:comment "5 25  Secretary may publish information given by holder of approved arrangement for exporter supply chain assurance operations - Abrievated Graph Key: I119"@en-AU ;
    skos:definition "5 25  Secretary may publish information given by holder of approved arrangement for exporter supply chain assurance operations"@en-AU ;
    skos:narrower F2021L00319:118 ;
    skos:prefLabel "Item I119"@en-AU ;
    dcat:accessURL <https://www.legislation.gov.au/F2021L00319/2024-04-30/2024-04-30/text/original/epub/OEBPS/document_1/document_1.html#_Toc166157952> ;
    dcat:landingPage "https://www.legislation.gov.au/F2021L00319/2024-04-30/2024-04-30/text/original/epub/OEBPS/document_1/document_1.html#_Toc166157952"^^xsd:anyURI ;
    dcat:theme legcons:Item .

F2021L00319:12 a legcons:Item,
        owl:Class,
        dcat:Resource ;
    rdfs:label "Item - I12 2 1  Livestock other live animals and animal reproductive material that are prescribed goods"@en-AU ;
    dct:isPartOf F2021L00319:11 ;
    dct:isReferencedBy F2021L00319: ;
    rdfs:comment "2 1  Livestock other live animals and animal reproductive material that are prescribed goods - Abrievated Graph Key: I12"@en-AU ;
    skos:definition "2 1  Livestock other live animals and animal reproductive material that are prescribed goods"@en-AU ;
    skos:narrower F2021L00319:11 ;
    skos:prefLabel "Item I12"@en-AU ;
    dcat:accessURL <https://www.legislation.gov.au/F2021L00319/2024-04-30/2024-04-30/text/original/epub/OEBPS/document_1/document_1.html#_Toc166157845> ;
    dcat:landingPage "https://www.legislation.gov.au/F2021L00319/2024-04-30/2024-04-30/text/original/epub/OEBPS/document_1/document_1.html#_Toc166157845"^^xsd:anyURI ;
    dcat:theme legcons:Item .

F2021L00319:121 a legcons:Item,
        owl:Class,
        dcat:Resource ;
    rdfs:label "Item - I121 5 26  Application of this Part"@en-AU ;
    dct:isPartOf F2021L00319:120 ;
    dct:isReferencedBy F2021L00319: ;
    rdfs:comment "5 26  Application of this Part - Abrievated Graph Key: I121"@en-AU ;
    skos:definition "5 26  Application of this Part"@en-AU ;
    skos:narrower F2021L00319:120 ;
    skos:prefLabel "Item I121"@en-AU ;
    dcat:accessURL <https://www.legislation.gov.au/F2021L00319/2024-04-30/2024-04-30/text/original/epub/OEBPS/document_1/document_1.html#_Toc166157954> ;
    dcat:landingPage "https://www.legislation.gov.au/F2021L00319/2024-04-30/2024-04-30/text/original/epub/OEBPS/document_1/document_1.html#_Toc166157954"^^xsd:anyURI ;
    dcat:theme legcons:Item .

F2021L00319:122 a legcons:Item,
        owl:Class,
        dcat:Resource ;
    rdfs:label "Item - I122 5 27  Documents to accompany application relating to arrangement for exporter supply chain assurance operations"@en-AU ;
    dct:isPartOf F2021L00319:120 ;
    dct:isReferencedBy F2021L00319: ;
    rdfs:comment "5 27  Documents to accompany application relating to arrangement for exporter supply chain assurance operations - Abrievated Graph Key: I122"@en-AU ;
    skos:definition "5 27  Documents to accompany application relating to arrangement for exporter supply chain assurance operations"@en-AU ;
    skos:narrower F2021L00319:120 ;
    skos:prefLabel "Item I122"@en-AU ;
    dcat:accessURL <https://www.legislation.gov.au/F2021L00319/2024-04-30/2024-04-30/text/original/epub/OEBPS/document_1/document_1.html#_Toc166157955> ;
    dcat:landingPage "https://www.legislation.gov.au/F2021L00319/2024-04-30/2024-04-30/text/original/epub/OEBPS/document_1/document_1.html#_Toc166157955"^^xsd:anyURI ;
    dcat:theme legcons:Item .

F2021L00319:123 a legcons:Item,
        owl:Class,
        dcat:Resource ;
    rdfs:label "Item - I123 5 28  Initial consideration period"@en-AU ;
    dct:isPartOf F2021L00319:120 ;
    dct:isReferencedBy F2021L00319: ;
    rdfs:comment "5 28  Initial consideration period - Abrievated Graph Key: I123"@en-AU ;
    skos:definition "5 28  Initial consideration period"@en-AU ;
    skos:narrower F2021L00319:120 ;
    skos:prefLabel "Item I123"@en-AU ;
    dcat:accessURL <https://www.legislation.gov.au/F2021L00319/2024-04-30/2024-04-30/text/original/epub/OEBPS/document_1/document_1.html#_Toc166157956> ;
    dcat:landingPage "https://www.legislation.gov.au/F2021L00319/2024-04-30/2024-04-30/text/original/epub/OEBPS/document_1/document_1.html#_Toc166157956"^^xsd:anyURI ;
    dcat:theme legcons:Item .

F2021L00319:124 a legcons:Item,
        owl:Class,
        dcat:Resource ;
    rdfs:label "Item - I124 5 29  Maximum period within which request relating to application must be complied with"@en-AU ;
    dct:isPartOf F2021L00319:120 ;
    dct:isReferencedBy F2021L00319: ;
    rdfs:comment "5 29  Maximum period within which request relating to application must be complied with - Abrievated Graph Key: I124"@en-AU ;
    skos:definition "5 29  Maximum period within which request relating to application must be complied with"@en-AU ;
    skos:narrower F2021L00319:120 ;
    skos:prefLabel "Item I124"@en-AU ;
    dcat:accessURL <https://www.legislation.gov.au/F2021L00319/2024-04-30/2024-04-30/text/original/epub/OEBPS/document_1/document_1.html#_Toc166157957> ;
    dcat:landingPage "https://www.legislation.gov.au/F2021L00319/2024-04-30/2024-04-30/text/original/epub/OEBPS/document_1/document_1.html#_Toc166157957"^^xsd:anyURI ;
    dcat:theme legcons:Item .

F2021L00319:128 a legcons:Item,
        owl:Class,
        dcat:Resource ;
    rdfs:label "Item - I128 6 1  Other requirements for grant of livestock export licence"@en-AU ;
    dct:isPartOf F2021L00319:127 ;
    dct:isReferencedBy F2021L00319: ;
    rdfs:comment "6 1  Other requirements for grant of livestock export licence - Abrievated Graph Key: I128"@en-AU ;
    skos:definition "6 1  Other requirements for grant of livestock export licence"@en-AU ;
    skos:narrower F2021L00319:127 ;
    skos:prefLabel "Item I128"@en-AU ;
    dcat:accessURL <https://www.legislation.gov.au/F2021L00319/2024-04-30/2024-04-30/text/original/epub/OEBPS/document_1/document_1.html#_Toc166157961> ;
    dcat:landingPage "https://www.legislation.gov.au/F2021L00319/2024-04-30/2024-04-30/text/original/epub/OEBPS/document_1/document_1.html#_Toc166157961"^^xsd:anyURI ;
    dcat:theme legcons:Item .

F2021L00319:13 a legcons:Division,
        owl:Class,
        dcat:Resource ;
    rdfs:label "Division - D13 Division 2 Prohibited export and prescribed export conditions"@en-AU ;
    dct:isPartOf F2021L00319:10 ;
    dct:isReferencedBy F2021L00319: ;
    rdfs:comment "Division 2 Prohibited export and prescribed export conditions - Abrievated Graph Key: D13"@en-AU ;
    skos:definition "Division 2 Prohibited export and prescribed export conditions"@en-AU ;
    skos:narrower F2021L00319:10 ;
    skos:prefLabel "Division D13"@en-AU ;
    dcat:accessURL <https://www.legislation.gov.au/F2021L00319/2024-04-30/2024-04-30/text/original/epub/OEBPS/document_1/document_1.html#_Toc166157846> ;
    dcat:landingPage "https://www.legislation.gov.au/F2021L00319/2024-04-30/2024-04-30/text/original/epub/OEBPS/document_1/document_1.html#_Toc166157846"^^xsd:anyURI ;
    dcat:theme legcons:Division .

F2021L00319:130 a legcons:Item,
        owl:Class,
        dcat:Resource ;
    rdfs:label "Item - I130 6 2  Other information to be stated in livestock export licence"@en-AU ;
    dct:isPartOf F2021L00319:129 ;
    dct:isReferencedBy F2021L00319: ;
    rdfs:comment "6 2  Other information to be stated in livestock export licence - Abrievated Graph Key: I130"@en-AU ;
    skos:definition "6 2  Other information to be stated in livestock export licence"@en-AU ;
    skos:narrower F2021L00319:129 ;
    skos:prefLabel "Item I130"@en-AU ;
    dcat:accessURL <https://www.legislation.gov.au/F2021L00319/2024-04-30/2024-04-30/text/original/epub/OEBPS/document_1/document_1.html#_Toc166157963> ;
    dcat:landingPage "https://www.legislation.gov.au/F2021L00319/2024-04-30/2024-04-30/text/original/epub/OEBPS/document_1/document_1.html#_Toc166157963"^^xsd:anyURI ;
    dcat:theme legcons:Item .

F2021L00319:131 a legcons:Item,
        owl:Class,
        dcat:Resource ;
    rdfs:label "Item - I131 6 3  Period of effect of livestock export licence"@en-AU ;
    dct:isPartOf F2021L00319:129 ;
    dct:isReferencedBy F2021L00319: ;
    rdfs:comment "6 3  Period of effect of livestock export licence - Abrievated Graph Key: I131"@en-AU ;
    skos:definition "6 3  Period of effect of livestock export licence"@en-AU ;
    skos:narrower F2021L00319:129 ;
    skos:prefLabel "Item I131"@en-AU ;
    dcat:accessURL <https://www.legislation.gov.au/F2021L00319/2024-04-30/2024-04-30/text/original/epub/OEBPS/document_1/document_1.html#_Toc166157964> ;
    dcat:landingPage "https://www.legislation.gov.au/F2021L00319/2024-04-30/2024-04-30/text/original/epub/OEBPS/document_1/document_1.html#_Toc166157964"^^xsd:anyURI ;
    dcat:theme legcons:Item .

F2021L00319:134 a legcons:Item,
        owl:Class,
        dcat:Resource ;
    rdfs:label "Item - I134 6 4  Purpose of this Part"@en-AU ;
    dct:isPartOf F2021L00319:133 ;
    dct:isReferencedBy F2021L00319: ;
    rdfs:comment "6 4  Purpose of this Part - Abrievated Graph Key: I134"@en-AU ;
    skos:definition "6 4  Purpose of this Part"@en-AU ;
    skos:narrower F2021L00319:133 ;
    skos:prefLabel "Item I134"@en-AU ;
    dcat:accessURL <https://www.legislation.gov.au/F2021L00319/2024-04-30/2024-04-30/text/original/epub/OEBPS/document_1/document_1.html#_Toc166157967> ;
    dcat:landingPage "https://www.legislation.gov.au/F2021L00319/2024-04-30/2024-04-30/text/original/epub/OEBPS/document_1/document_1.html#_Toc166157967"^^xsd:anyURI ;
    dcat:theme legcons:Item .

F2021L00319:136 a legcons:Item,
        owl:Class,
        dcat:Resource ;
    rdfs:label "Item - I136 6 5  Audits"@en-AU ;
    dct:isPartOf F2021L00319:135 ;
    dct:isReferencedBy F2021L00319: ;
    rdfs:comment "6 5  Audits - Abrievated Graph Key: I136"@en-AU ;
    skos:definition "6 5  Audits"@en-AU ;
    skos:narrower F2021L00319:135 ;
    skos:prefLabel "Item I136"@en-AU ;
    dcat:accessURL <https://www.legislation.gov.au/F2021L00319/2024-04-30/2024-04-30/text/original/epub/OEBPS/document_1/document_1.html#_Toc166157969> ;
    dcat:landingPage "https://www.legislation.gov.au/F2021L00319/2024-04-30/2024-04-30/text/original/epub/OEBPS/document_1/document_1.html#_Toc166157969"^^xsd:anyURI ;
    dcat:theme legcons:Item .

F2021L00319:137 a legcons:Item,
        owl:Class,
        dcat:Resource ;
    rdfs:label "Item - I137 6 6  Australian Standards for the Export of Livestock"@en-AU ;
    dct:isPartOf F2021L00319:135 ;
    dct:isReferencedBy F2021L00319: ;
    rdfs:comment "6 6  Australian Standards for the Export of Livestock - Abrievated Graph Key: I137"@en-AU ;
    skos:definition "6 6  Australian Standards for the Export of Livestock"@en-AU ;
    skos:narrower F2021L00319:135 ;
    skos:prefLabel "Item I137"@en-AU ;
    dcat:accessURL <https://www.legislation.gov.au/F2021L00319/2024-04-30/2024-04-30/text/original/epub/OEBPS/document_1/document_1.html#_Toc166157970> ;
    dcat:landingPage "https://www.legislation.gov.au/F2021L00319/2024-04-30/2024-04-30/text/original/epub/OEBPS/document_1/document_1.html#_Toc166157970"^^xsd:anyURI ;
    dcat:theme legcons:Item .

F2021L00319:138 a legcons:Item,
        owl:Class,
        dcat:Resource ;
    rdfs:label "Item - I138 6 7  Holder of licence must have and comply with an approved ESCAS"@en-AU ;
    dct:isPartOf F2021L00319:135 ;
    dct:isReferencedBy F2021L00319: ;
    rdfs:comment "6 7  Holder of licence must have and comply with an approved ESCAS - Abrievated Graph Key: I138"@en-AU ;
    skos:definition "6 7  Holder of licence must have and comply with an approved ESCAS"@en-AU ;
    skos:narrower F2021L00319:135 ;
    skos:prefLabel "Item I138"@en-AU ;
    dcat:accessURL <https://www.legislation.gov.au/F2021L00319/2024-04-30/2024-04-30/text/original/epub/OEBPS/document_1/document_1.html#_Toc166157971> ;
    dcat:landingPage "https://www.legislation.gov.au/F2021L00319/2024-04-30/2024-04-30/text/original/epub/OEBPS/document_1/document_1.html#_Toc166157971"^^xsd:anyURI ;
    dcat:theme legcons:Item .

F2021L00319:139 a legcons:Item,
        owl:Class,
        dcat:Resource ;
    rdfs:label "Item - I139 6 8  Compliance with operations and governance manual"@en-AU ;
    dct:isPartOf F2021L00319:135 ;
    dct:isReferencedBy F2021L00319: ;
    rdfs:comment "6 8  Compliance with operations and governance manual - Abrievated Graph Key: I139"@en-AU ;
    skos:definition "6 8  Compliance with operations and governance manual"@en-AU ;
    skos:narrower F2021L00319:135 ;
    skos:prefLabel "Item I139"@en-AU ;
    dcat:accessURL <https://www.legislation.gov.au/F2021L00319/2024-04-30/2024-04-30/text/original/epub/OEBPS/document_1/document_1.html#_Toc166157972> ;
    dcat:landingPage "https://www.legislation.gov.au/F2021L00319/2024-04-30/2024-04-30/text/original/epub/OEBPS/document_1/document_1.html#_Toc166157972"^^xsd:anyURI ;
    dcat:theme legcons:Item .

F2021L00319:14 a legcons:Item,
        owl:Class,
        dcat:Resource ;
    rdfs:label "Item - I14 2 2  Purpose and application of this Division"@en-AU ;
    dct:isPartOf F2021L00319:10 ;
    dct:isReferencedBy F2021L00319: ;
    rdfs:comment "2 2  Purpose and application of this Division - Abrievated Graph Key: I14"@en-AU ;
    skos:definition "2 2  Purpose and application of this Division"@en-AU ;
    skos:narrower F2021L00319:10 ;
    skos:prefLabel "Item I14"@en-AU ;
    dcat:accessURL <https://www.legislation.gov.au/F2021L00319/2024-04-30/2024-04-30/text/original/epub/OEBPS/document_1/document_1.html#_Toc166157847> ;
    dcat:landingPage "https://www.legislation.gov.au/F2021L00319/2024-04-30/2024-04-30/text/original/epub/OEBPS/document_1/document_1.html#_Toc166157847"^^xsd:anyURI ;
    dcat:theme legcons:Item .

F2021L00319:140 a legcons:Item,
        owl:Class,
        dcat:Resource ;
    rdfs:label "Item - I140 6 8 A  Orders made by authorised officer"@en-AU ;
    dct:isPartOf F2021L00319:135 ;
    dct:isReferencedBy F2021L00319: ;
    rdfs:comment "6 8 A  Orders made by authorised officer - Abrievated Graph Key: I140"@en-AU ;
    skos:definition "6 8 A  Orders made by authorised officer"@en-AU ;
    skos:narrower F2021L00319:135 ;
    skos:prefLabel "Item I140"@en-AU ;
    dcat:accessURL <https://www.legislation.gov.au/F2021L00319/2024-04-30/2024-04-30/text/original/epub/OEBPS/document_1/document_1.html#_Toc166157973> ;
    dcat:landingPage "https://www.legislation.gov.au/F2021L00319/2024-04-30/2024-04-30/text/original/epub/OEBPS/document_1/document_1.html#_Toc166157973"^^xsd:anyURI ;
    dcat:theme legcons:Item .

F2021L00319:142 a legcons:Item,
        owl:Class,
        dcat:Resource ;
    rdfs:label "Item - I142 6 9  Restrictions on export"@en-AU ;
    dct:isPartOf F2021L00319:141 ;
    dct:isReferencedBy F2021L00319: ;
    rdfs:comment "6 9  Restrictions on export - Abrievated Graph Key: I142"@en-AU ;
    skos:definition "6 9  Restrictions on export"@en-AU ;
    skos:narrower F2021L00319:141 ;
    skos:prefLabel "Item I142"@en-AU ;
    dcat:accessURL <https://www.legislation.gov.au/F2021L00319/2024-04-30/2024-04-30/text/original/epub/OEBPS/document_1/document_1.html#_Toc166157975> ;
    dcat:landingPage "https://www.legislation.gov.au/F2021L00319/2024-04-30/2024-04-30/text/original/epub/OEBPS/document_1/document_1.html#_Toc166157975"^^xsd:anyURI ;
    dcat:theme legcons:Item .

F2021L00319:143 a legcons:Item,
        owl:Class,
        dcat:Resource ;
    rdfs:label "Item - I143 6 10  Conditions on export"@en-AU ;
    dct:isPartOf F2021L00319:141 ;
    dct:isReferencedBy F2021L00319: ;
    rdfs:comment "6 10  Conditions on export - Abrievated Graph Key: I143"@en-AU ;
    skos:definition "6 10  Conditions on export"@en-AU ;
    skos:narrower F2021L00319:141 ;
    skos:prefLabel "Item I143"@en-AU ;
    dcat:accessURL <https://www.legislation.gov.au/F2021L00319/2024-04-30/2024-04-30/text/original/epub/OEBPS/document_1/document_1.html#_Toc166157976> ;
    dcat:landingPage "https://www.legislation.gov.au/F2021L00319/2024-04-30/2024-04-30/text/original/epub/OEBPS/document_1/document_1.html#_Toc166157976"^^xsd:anyURI ;
    dcat:theme legcons:Item .

F2021L00319:146 a legcons:Item,
        owl:Class,
        dcat:Resource ;
    rdfs:label "Item - I146 6 11  Application of this Division"@en-AU ;
    dct:isPartOf F2021L00319:145 ;
    dct:isReferencedBy F2021L00319: ;
    rdfs:comment "6 11  Application of this Division - Abrievated Graph Key: I146"@en-AU ;
    skos:definition "6 11  Application of this Division"@en-AU ;
    skos:narrower F2021L00319:145 ;
    skos:prefLabel "Item I146"@en-AU ;
    dcat:accessURL <https://www.legislation.gov.au/F2021L00319/2024-04-30/2024-04-30/text/original/epub/OEBPS/document_1/document_1.html#_Toc166157979> ;
    dcat:landingPage "https://www.legislation.gov.au/F2021L00319/2024-04-30/2024-04-30/text/original/epub/OEBPS/document_1/document_1.html#_Toc166157979"^^xsd:anyURI ;
    dcat:theme legcons:Item .

F2021L00319:147 a legcons:Subdivision,
        owl:Class,
        dcat:Resource ;
    rdfs:label "Subdivision - S147 Subdivision BProhibition on export to specific places"@en-AU ;
    dct:isPartOf F2021L00319:144 ;
    dct:isReferencedBy F2021L00319: ;
    rdfs:comment "Subdivision BProhibition on export to specific places - Abrievated Graph Key: S147"@en-AU ;
    skos:definition "Subdivision BProhibition on export to specific places"@en-AU ;
    skos:narrower F2021L00319:144 ;
    skos:prefLabel "Subdivision S147"@en-AU ;
    dcat:accessURL <https://www.legislation.gov.au/F2021L00319/2024-04-30/2024-04-30/text/original/epub/OEBPS/document_1/document_1.html#_Toc166157980> ;
    dcat:landingPage "https://www.legislation.gov.au/F2021L00319/2024-04-30/2024-04-30/text/original/epub/OEBPS/document_1/document_1.html#_Toc166157980"^^xsd:anyURI ;
    dcat:theme legcons:Subdivision .

F2021L00319:148 a legcons:Item,
        owl:Class,
        dcat:Resource ;
    rdfs:label "Item - I148 6 12  Sheep must not be exported to Oman between 8 May and 14 September"@en-AU ;
    dct:isPartOf F2021L00319:144 ;
    dct:isReferencedBy F2021L00319: ;
    rdfs:comment "6 12  Sheep must not be exported to Oman between 8 May and 14 September - Abrievated Graph Key: I148"@en-AU ;
    skos:definition "6 12  Sheep must not be exported to Oman between 8 May and 14 September"@en-AU ;
    skos:narrower F2021L00319:144 ;
    skos:prefLabel "Item I148"@en-AU ;
    dcat:accessURL <https://www.legislation.gov.au/F2021L00319/2024-04-30/2024-04-30/text/original/epub/OEBPS/document_1/document_1.html#_Toc166157981> ;
    dcat:landingPage "https://www.legislation.gov.au/F2021L00319/2024-04-30/2024-04-30/text/original/epub/OEBPS/document_1/document_1.html#_Toc166157981"^^xsd:anyURI ;
    dcat:theme legcons:Item .

F2021L00319:149 a legcons:Item,
        owl:Class,
        dcat:Resource ;
    rdfs:label "Item - I149 6 13  Sheep must not be exported to Qatar between 1 June and 21 September"@en-AU ;
    dct:isPartOf F2021L00319:144 ;
    dct:isReferencedBy F2021L00319: ;
    rdfs:comment "6 13  Sheep must not be exported to Qatar between 1 June and 21 September - Abrievated Graph Key: I149"@en-AU ;
    skos:definition "6 13  Sheep must not be exported to Qatar between 1 June and 21 September"@en-AU ;
    skos:narrower F2021L00319:144 ;
    skos:prefLabel "Item I149"@en-AU ;
    dcat:accessURL <https://www.legislation.gov.au/F2021L00319/2024-04-30/2024-04-30/text/original/epub/OEBPS/document_1/document_1.html#_Toc166157982> ;
    dcat:landingPage "https://www.legislation.gov.au/F2021L00319/2024-04-30/2024-04-30/text/original/epub/OEBPS/document_1/document_1.html#_Toc166157982"^^xsd:anyURI ;
    dcat:theme legcons:Item .

F2021L00319:15 a legcons:Item,
        owl:Class,
        dcat:Resource ;
    rdfs:label "Item - I15 2 3  Export of prescribed livestock is prohibited unless prescribed conditions are complied with"@en-AU ;
    dct:isPartOf F2021L00319:10 ;
    dct:isReferencedBy F2021L00319: ;
    rdfs:comment "2 3  Export of prescribed livestock is prohibited unless prescribed conditions are complied with - Abrievated Graph Key: I15"@en-AU ;
    skos:definition "2 3  Export of prescribed livestock is prohibited unless prescribed conditions are complied with"@en-AU ;
    skos:narrower F2021L00319:10 ;
    skos:prefLabel "Item I15"@en-AU ;
    dcat:accessURL <https://www.legislation.gov.au/F2021L00319/2024-04-30/2024-04-30/text/original/epub/OEBPS/document_1/document_1.html#_Toc166157848> ;
    dcat:landingPage "https://www.legislation.gov.au/F2021L00319/2024-04-30/2024-04-30/text/original/epub/OEBPS/document_1/document_1.html#_Toc166157848"^^xsd:anyURI ;
    dcat:theme legcons:Item .

F2021L00319:150 a legcons:Item,
        owl:Class,
        dcat:Resource ;
    rdfs:label "Item - I150 6 14  Sheep must not be exported to Bahrain Iran Iraq Kingdom of Saudi Arabia Kuwait or the United Arab Emirates between 1 June and 14 September"@en-AU ;
    dct:isPartOf F2021L00319:144 ;
    dct:isReferencedBy F2021L00319: ;
    rdfs:comment "6 14  Sheep must not be exported to Bahrain Iran Iraq Kingdom of Saudi Arabia Kuwait or the United Arab Emirates between 1 June and 14 September - Abrievated Graph Key: I150"@en-AU ;
    skos:definition "6 14  Sheep must not be exported to Bahrain Iran Iraq Kingdom of Saudi Arabia Kuwait or the United Arab Emirates between 1 June and 14 September"@en-AU ;
    skos:narrower F2021L00319:144 ;
    skos:prefLabel "Item I150"@en-AU ;
    dcat:accessURL <https://www.legislation.gov.au/F2021L00319/2024-04-30/2024-04-30/text/original/epub/OEBPS/document_1/document_1.html#_Toc166157983> ;
    dcat:landingPage "https://www.legislation.gov.au/F2021L00319/2024-04-30/2024-04-30/text/original/epub/OEBPS/document_1/document_1.html#_Toc166157983"^^xsd:anyURI ;
    dcat:theme legcons:Item .

F2021L00319:151 a legcons:Item,
        owl:Class,
        dcat:Resource ;
    rdfs:label "Item - I151 6 14 A  Sheep must not be exported through certain waters between 15 June and 14 September"@en-AU ;
    dct:isPartOf F2021L00319:144 ;
    dct:isReferencedBy F2021L00319: ;
    rdfs:comment "6 14 A  Sheep must not be exported through certain waters between 15 June and 14 September - Abrievated Graph Key: I151"@en-AU ;
    skos:definition "6 14 A  Sheep must not be exported through certain waters between 15 June and 14 September"@en-AU ;
    skos:narrower F2021L00319:144 ;
    skos:prefLabel "Item I151"@en-AU ;
    dcat:accessURL <https://www.legislation.gov.au/F2021L00319/2024-04-30/2024-04-30/text/original/epub/OEBPS/document_1/document_1.html#_Toc166157984> ;
    dcat:landingPage "https://www.legislation.gov.au/F2021L00319/2024-04-30/2024-04-30/text/original/epub/OEBPS/document_1/document_1.html#_Toc166157984"^^xsd:anyURI ;
    dcat:theme legcons:Item .

F2021L00319:152 a legcons:Item,
        owl:Class,
        dcat:Resource ;
    rdfs:label "Item - I152 6 14 B  Sheep must not be exported to certain countries in the Middle East between 22 May and 31 May unless certain conditions satisfied"@en-AU ;
    dct:isPartOf F2021L00319:144 ;
    dct:isReferencedBy F2021L00319: ;
    rdfs:comment "6 14 B  Sheep must not be exported to certain countries in the Middle East between 22 May and 31 May unless certain conditions satisfied - Abrievated Graph Key: I152"@en-AU ;
    skos:definition "6 14 B  Sheep must not be exported to certain countries in the Middle East between 22 May and 31 May unless certain conditions satisfied"@en-AU ;
    skos:narrower F2021L00319:144 ;
    skos:prefLabel "Item I152"@en-AU ;
    dcat:accessURL <https://www.legislation.gov.au/F2021L00319/2024-04-30/2024-04-30/text/original/epub/OEBPS/document_1/document_1.html#_Toc166157985> ;
    dcat:landingPage "https://www.legislation.gov.au/F2021L00319/2024-04-30/2024-04-30/text/original/epub/OEBPS/document_1/document_1.html#_Toc166157985"^^xsd:anyURI ;
    dcat:theme legcons:Item .

F2021L00319:153 a legcons:Subdivision,
        owl:Class,
        dcat:Resource ;
    rdfs:label "Subdivision - S153 Subdivision CExports during northern summer"@en-AU ;
    dct:isPartOf F2021L00319:144 ;
    dct:isReferencedBy F2021L00319: ;
    rdfs:comment "Subdivision CExports during northern summer - Abrievated Graph Key: S153"@en-AU ;
    skos:definition "Subdivision CExports during northern summer"@en-AU ;
    skos:narrower F2021L00319:144 ;
    skos:prefLabel "Subdivision S153"@en-AU ;
    dcat:accessURL <https://www.legislation.gov.au/F2021L00319/2024-04-30/2024-04-30/text/original/epub/OEBPS/document_1/document_1.html#_Toc166157986> ;
    dcat:landingPage "https://www.legislation.gov.au/F2021L00319/2024-04-30/2024-04-30/text/original/epub/OEBPS/document_1/document_1.html#_Toc166157986"^^xsd:anyURI ;
    dcat:theme legcons:Subdivision .

F2021L00319:154 a legcons:Item,
        owl:Class,
        dcat:Resource ;
    rdfs:label "Item - I154 6 15  Application of this Subdivision"@en-AU ;
    dct:isPartOf F2021L00319:144 ;
    dct:isReferencedBy F2021L00319: ;
    rdfs:comment "6 15  Application of this Subdivision - Abrievated Graph Key: I154"@en-AU ;
    skos:definition "6 15  Application of this Subdivision"@en-AU ;
    skos:narrower F2021L00319:144 ;
    skos:prefLabel "Item I154"@en-AU ;
    dcat:accessURL <https://www.legislation.gov.au/F2021L00319/2024-04-30/2024-04-30/text/original/epub/OEBPS/document_1/document_1.html#_Toc166157987> ;
    dcat:landingPage "https://www.legislation.gov.au/F2021L00319/2024-04-30/2024-04-30/text/original/epub/OEBPS/document_1/document_1.html#_Toc166157987"^^xsd:anyURI ;
    dcat:theme legcons:Item .

F2021L00319:155 a legcons:Item,
        owl:Class,
        dcat:Resource ;
    rdfs:label "Item - I155 6 16  General conditions"@en-AU ;
    dct:isPartOf F2021L00319:144 ;
    dct:isReferencedBy F2021L00319: ;
    rdfs:comment "6 16  General conditions - Abrievated Graph Key: I155"@en-AU ;
    skos:definition "6 16  General conditions"@en-AU ;
    skos:narrower F2021L00319:144 ;
    skos:prefLabel "Item I155"@en-AU ;
    dcat:accessURL <https://www.legislation.gov.au/F2021L00319/2024-04-30/2024-04-30/text/original/epub/OEBPS/document_1/document_1.html#_Toc166157988> ;
    dcat:landingPage "https://www.legislation.gov.au/F2021L00319/2024-04-30/2024-04-30/text/original/epub/OEBPS/document_1/document_1.html#_Toc166157988"^^xsd:anyURI ;
    dcat:theme legcons:Item .

F2021L00319:156 a legcons:Item,
        owl:Class,
        dcat:Resource ;
    rdfs:label "Item - I156 6 17  Pen air turnover"@en-AU ;
    dct:isPartOf F2021L00319:144 ;
    dct:isReferencedBy F2021L00319: ;
    rdfs:comment "6 17  Pen air turnover - Abrievated Graph Key: I156"@en-AU ;
    skos:definition "6 17  Pen air turnover"@en-AU ;
    skos:narrower F2021L00319:144 ;
    skos:prefLabel "Item I156"@en-AU ;
    dcat:accessURL <https://www.legislation.gov.au/F2021L00319/2024-04-30/2024-04-30/text/original/epub/OEBPS/document_1/document_1.html#_Toc166157989> ;
    dcat:landingPage "https://www.legislation.gov.au/F2021L00319/2024-04-30/2024-04-30/text/original/epub/OEBPS/document_1/document_1.html#_Toc166157989"^^xsd:anyURI ;
    dcat:theme legcons:Item .

F2021L00319:157 a legcons:Item,
        owl:Class,
        dcat:Resource ;
    rdfs:label "Item - I157 6 18  Condition of sheep and of pens on vessel"@en-AU ;
    dct:isPartOf F2021L00319:144 ;
    dct:isReferencedBy F2021L00319: ;
    rdfs:comment "6 18  Condition of sheep and of pens on vessel - Abrievated Graph Key: I157"@en-AU ;
    skos:definition "6 18  Condition of sheep and of pens on vessel"@en-AU ;
    skos:narrower F2021L00319:144 ;
    skos:prefLabel "Item I157"@en-AU ;
    dcat:accessURL <https://www.legislation.gov.au/F2021L00319/2024-04-30/2024-04-30/text/original/epub/OEBPS/document_1/document_1.html#_Toc166157990> ;
    dcat:landingPage "https://www.legislation.gov.au/F2021L00319/2024-04-30/2024-04-30/text/original/epub/OEBPS/document_1/document_1.html#_Toc166157990"^^xsd:anyURI ;
    dcat:theme legcons:Item .

F2021L00319:158 a legcons:Item,
        owl:Class,
        dcat:Resource ;
    rdfs:label "Item - I158 6 19  Exports to Kuwait"@en-AU ;
    dct:isPartOf F2021L00319:144 ;
    dct:isReferencedBy F2021L00319: ;
    rdfs:comment "6 19  Exports to Kuwait - Abrievated Graph Key: I158"@en-AU ;
    skos:definition "6 19  Exports to Kuwait"@en-AU ;
    skos:narrower F2021L00319:144 ;
    skos:prefLabel "Item I158"@en-AU ;
    dcat:accessURL <https://www.legislation.gov.au/F2021L00319/2024-04-30/2024-04-30/text/original/epub/OEBPS/document_1/document_1.html#_Toc166157991> ;
    dcat:landingPage "https://www.legislation.gov.au/F2021L00319/2024-04-30/2024-04-30/text/original/epub/OEBPS/document_1/document_1.html#_Toc166157991"^^xsd:anyURI ;
    dcat:theme legcons:Item .

F2021L00319:159 a legcons:Item,
        owl:Class,
        dcat:Resource ;
    rdfs:label "Item - I159 6 19 A  Conditions that apply in relation to the export of sheep between 1 May and 14 Junecertain voyages"@en-AU ;
    dct:isPartOf F2021L00319:144 ;
    dct:isReferencedBy F2021L00319: ;
    rdfs:comment "6 19 A  Conditions that apply in relation to the export of sheep between 1 May and 14 Junecertain voyages - Abrievated Graph Key: I159"@en-AU ;
    skos:definition "6 19 A  Conditions that apply in relation to the export of sheep between 1 May and 14 Junecertain voyages"@en-AU ;
    skos:narrower F2021L00319:144 ;
    skos:prefLabel "Item I159"@en-AU ;
    dcat:accessURL <https://www.legislation.gov.au/F2021L00319/2024-04-30/2024-04-30/text/original/epub/OEBPS/document_1/document_1.html#_Toc166157992> ;
    dcat:landingPage "https://www.legislation.gov.au/F2021L00319/2024-04-30/2024-04-30/text/original/epub/OEBPS/document_1/document_1.html#_Toc166157992"^^xsd:anyURI ;
    dcat:theme legcons:Item .

F2021L00319:16 a legcons:Item,
        owl:Class,
        dcat:Resource ;
    rdfs:label "Item - I16 2 4  Export of prescribed live animals is prohibited unless prescribed conditions are complied with"@en-AU ;
    dct:isPartOf F2021L00319:10 ;
    dct:isReferencedBy F2021L00319: ;
    rdfs:comment "2 4  Export of prescribed live animals is prohibited unless prescribed conditions are complied with - Abrievated Graph Key: I16"@en-AU ;
    skos:definition "2 4  Export of prescribed live animals is prohibited unless prescribed conditions are complied with"@en-AU ;
    skos:narrower F2021L00319:10 ;
    skos:prefLabel "Item I16"@en-AU ;
    dcat:accessURL <https://www.legislation.gov.au/F2021L00319/2024-04-30/2024-04-30/text/original/epub/OEBPS/document_1/document_1.html#_Toc166157849> ;
    dcat:landingPage "https://www.legislation.gov.au/F2021L00319/2024-04-30/2024-04-30/text/original/epub/OEBPS/document_1/document_1.html#_Toc166157849"^^xsd:anyURI ;
    dcat:theme legcons:Item .

F2021L00319:160 a legcons:Item,
        owl:Class,
        dcat:Resource ;
    rdfs:label "Item - I160 6 20  Restrictions on number of ports where vessel may dockcertain voyages"@en-AU ;
    dct:isPartOf F2021L00319:144 ;
    dct:isReferencedBy F2021L00319: ;
    rdfs:comment "6 20  Restrictions on number of ports where vessel may dockcertain voyages - Abrievated Graph Key: I160"@en-AU ;
    skos:definition "6 20  Restrictions on number of ports where vessel may dockcertain voyages"@en-AU ;
    skos:narrower F2021L00319:144 ;
    skos:prefLabel "Item I160"@en-AU ;
    dcat:accessURL <https://www.legislation.gov.au/F2021L00319/2024-04-30/2024-04-30/text/original/epub/OEBPS/document_1/document_1.html#_Toc166157993> ;
    dcat:landingPage "https://www.legislation.gov.au/F2021L00319/2024-04-30/2024-04-30/text/original/epub/OEBPS/document_1/document_1.html#_Toc166157993"^^xsd:anyURI ;
    dcat:theme legcons:Item .

F2021L00319:161 a legcons:Subdivision,
        owl:Class,
        dcat:Resource ;
    rdfs:label "Subdivision - S161 Subdivision DExports during northern winter"@en-AU ;
    dct:isPartOf F2021L00319:144 ;
    dct:isReferencedBy F2021L00319: ;
    rdfs:comment "Subdivision DExports during northern winter - Abrievated Graph Key: S161"@en-AU ;
    skos:definition "Subdivision DExports during northern winter"@en-AU ;
    skos:narrower F2021L00319:144 ;
    skos:prefLabel "Subdivision S161"@en-AU ;
    dcat:accessURL <https://www.legislation.gov.au/F2021L00319/2024-04-30/2024-04-30/text/original/epub/OEBPS/document_1/document_1.html#_Toc166157994> ;
    dcat:landingPage "https://www.legislation.gov.au/F2021L00319/2024-04-30/2024-04-30/text/original/epub/OEBPS/document_1/document_1.html#_Toc166157994"^^xsd:anyURI ;
    dcat:theme legcons:Subdivision .

F2021L00319:162 a legcons:Item,
        owl:Class,
        dcat:Resource ;
    rdfs:label "Item - I162 6 21  Application of this Subdivision"@en-AU ;
    dct:isPartOf F2021L00319:144 ;
    dct:isReferencedBy F2021L00319: ;
    rdfs:comment "6 21  Application of this Subdivision - Abrievated Graph Key: I162"@en-AU ;
    skos:definition "6 21  Application of this Subdivision"@en-AU ;
    skos:narrower F2021L00319:144 ;
    skos:prefLabel "Item I162"@en-AU ;
    dcat:accessURL <https://www.legislation.gov.au/F2021L00319/2024-04-30/2024-04-30/text/original/epub/OEBPS/document_1/document_1.html#_Toc166157995> ;
    dcat:landingPage "https://www.legislation.gov.au/F2021L00319/2024-04-30/2024-04-30/text/original/epub/OEBPS/document_1/document_1.html#_Toc166157995"^^xsd:anyURI ;
    dcat:theme legcons:Item .

F2021L00319:163 a legcons:Item,
        owl:Class,
        dcat:Resource ;
    rdfs:label "Item - I163 6 22  Watering systems"@en-AU ;
    dct:isPartOf F2021L00319:144 ;
    dct:isReferencedBy F2021L00319: ;
    rdfs:comment "6 22  Watering systems - Abrievated Graph Key: I163"@en-AU ;
    skos:definition "6 22  Watering systems"@en-AU ;
    skos:narrower F2021L00319:144 ;
    skos:prefLabel "Item I163"@en-AU ;
    dcat:accessURL <https://www.legislation.gov.au/F2021L00319/2024-04-30/2024-04-30/text/original/epub/OEBPS/document_1/document_1.html#_Toc166157996> ;
    dcat:landingPage "https://www.legislation.gov.au/F2021L00319/2024-04-30/2024-04-30/text/original/epub/OEBPS/document_1/document_1.html#_Toc166157996"^^xsd:anyURI ;
    dcat:theme legcons:Item .

F2021L00319:164 a legcons:Item,
        owl:Class,
        dcat:Resource ;
    rdfs:label "Item - I164 6 23  Pen air turnover"@en-AU ;
    dct:isPartOf F2021L00319:144 ;
    dct:isReferencedBy F2021L00319: ;
    rdfs:comment "6 23  Pen air turnover - Abrievated Graph Key: I164"@en-AU ;
    skos:definition "6 23  Pen air turnover"@en-AU ;
    skos:narrower F2021L00319:144 ;
    skos:prefLabel "Item I164"@en-AU ;
    dcat:accessURL <https://www.legislation.gov.au/F2021L00319/2024-04-30/2024-04-30/text/original/epub/OEBPS/document_1/document_1.html#_Toc166157997> ;
    dcat:landingPage "https://www.legislation.gov.au/F2021L00319/2024-04-30/2024-04-30/text/original/epub/OEBPS/document_1/document_1.html#_Toc166157997"^^xsd:anyURI ;
    dcat:theme legcons:Item .

F2021L00319:165 a legcons:Division,
        owl:Class,
        dcat:Resource ;
    rdfs:label "Division - D165 Division 5 Exports of sheep goats and cattle to the Kingdom of Saudi Arabia"@en-AU ;
    dct:isPartOf F2021L00319:132 ;
    dct:isReferencedBy F2021L00319: ;
    rdfs:comment "Division 5 Exports of sheep goats and cattle to the Kingdom of Saudi Arabia - Abrievated Graph Key: D165"@en-AU ;
    skos:definition "Division 5 Exports of sheep goats and cattle to the Kingdom of Saudi Arabia"@en-AU ;
    skos:narrower F2021L00319:132 ;
    skos:prefLabel "Division D165"@en-AU ;
    dcat:accessURL <https://www.legislation.gov.au/F2021L00319/2024-04-30/2024-04-30/text/original/epub/OEBPS/document_1/document_1.html#_Toc166157998> ;
    dcat:landingPage "https://www.legislation.gov.au/F2021L00319/2024-04-30/2024-04-30/text/original/epub/OEBPS/document_1/document_1.html#_Toc166157998"^^xsd:anyURI ;
    dcat:theme legcons:Division .

F2021L00319:166 a legcons:Item,
        owl:Class,
        dcat:Resource ;
    rdfs:label "Item - I166 6 24  Pre export conditions for sheep and goats"@en-AU ;
    dct:isPartOf F2021L00319:132 ;
    dct:isReferencedBy F2021L00319: ;
    rdfs:comment "6 24  Pre export conditions for sheep and goats - Abrievated Graph Key: I166"@en-AU ;
    skos:definition "6 24  Pre export conditions for sheep and goats"@en-AU ;
    skos:narrower F2021L00319:132 ;
    skos:prefLabel "Item I166"@en-AU ;
    dcat:accessURL <https://www.legislation.gov.au/F2021L00319/2024-04-30/2024-04-30/text/original/epub/OEBPS/document_1/document_1.html#_Toc166157999> ;
    dcat:landingPage "https://www.legislation.gov.au/F2021L00319/2024-04-30/2024-04-30/text/original/epub/OEBPS/document_1/document_1.html#_Toc166157999"^^xsd:anyURI ;
    dcat:theme legcons:Item .

F2021L00319:167 a legcons:Item,
        owl:Class,
        dcat:Resource ;
    rdfs:label "Item - I167 6 25  Shipping conditions for sheep goats and cattle"@en-AU ;
    dct:isPartOf F2021L00319:132 ;
    dct:isReferencedBy F2021L00319: ;
    rdfs:comment "6 25  Shipping conditions for sheep goats and cattle - Abrievated Graph Key: I167"@en-AU ;
    skos:definition "6 25  Shipping conditions for sheep goats and cattle"@en-AU ;
    skos:narrower F2021L00319:132 ;
    skos:prefLabel "Item I167"@en-AU ;
    dcat:accessURL <https://www.legislation.gov.au/F2021L00319/2024-04-30/2024-04-30/text/original/epub/OEBPS/document_1/document_1.html#_Toc166158000> ;
    dcat:landingPage "https://www.legislation.gov.au/F2021L00319/2024-04-30/2024-04-30/text/original/epub/OEBPS/document_1/document_1.html#_Toc166158000"^^xsd:anyURI ;
    dcat:theme legcons:Item .

F2021L00319:168 a legcons:Part,
        owl:Class,
        dcat:Resource ;
    rdfs:label "Part - P168 Part 3 Renewal of livestock export licence"@en-AU ;
    dct:isPartOf F2021L00319:125 ;
    dct:isReferencedBy F2021L00319: ;
    rdfs:comment "Part 3 Renewal of livestock export licence - Abrievated Graph Key: P168"@en-AU ;
    skos:definition "Part 3 Renewal of livestock export licence"@en-AU ;
    skos:narrower F2021L00319:125 ;
    skos:prefLabel "Part P168"@en-AU ;
    dcat:accessURL <https://www.legislation.gov.au/F2021L00319/2024-04-30/2024-04-30/text/original/epub/OEBPS/document_1/document_1.html#_Toc166158001> ;
    dcat:landingPage "https://www.legislation.gov.au/F2021L00319/2024-04-30/2024-04-30/text/original/epub/OEBPS/document_1/document_1.html#_Toc166158001"^^xsd:anyURI ;
    dcat:theme legcons:Part .

F2021L00319:169 a legcons:Item,
        owl:Class,
        dcat:Resource ;
    rdfs:label "Item - I169 6 26  Period within which application to renew livestock export licence must be made"@en-AU ;
    dct:isPartOf F2021L00319:125 ;
    dct:isReferencedBy F2021L00319: ;
    rdfs:comment "6 26  Period within which application to renew livestock export licence must be made - Abrievated Graph Key: I169"@en-AU ;
    skos:definition "6 26  Period within which application to renew livestock export licence must be made"@en-AU ;
    skos:narrower F2021L00319:125 ;
    skos:prefLabel "Item I169"@en-AU ;
    dcat:accessURL <https://www.legislation.gov.au/F2021L00319/2024-04-30/2024-04-30/text/original/epub/OEBPS/document_1/document_1.html#_Toc166158002> ;
    dcat:landingPage "https://www.legislation.gov.au/F2021L00319/2024-04-30/2024-04-30/text/original/epub/OEBPS/document_1/document_1.html#_Toc166158002"^^xsd:anyURI ;
    dcat:theme legcons:Item .

F2021L00319:17 a legcons:Item,
        owl:Class,
        dcat:Resource ;
    rdfs:label "Item - I17 2 5  Export of prescribed animal reproductive material is prohibited unless prescribed conditions are complied with"@en-AU ;
    dct:isPartOf F2021L00319:10 ;
    dct:isReferencedBy F2021L00319: ;
    rdfs:comment "2 5  Export of prescribed animal reproductive material is prohibited unless prescribed conditions are complied with - Abrievated Graph Key: I17"@en-AU ;
    skos:definition "2 5  Export of prescribed animal reproductive material is prohibited unless prescribed conditions are complied with"@en-AU ;
    skos:narrower F2021L00319:10 ;
    skos:prefLabel "Item I17"@en-AU ;
    dcat:accessURL <https://www.legislation.gov.au/F2021L00319/2024-04-30/2024-04-30/text/original/epub/OEBPS/document_1/document_1.html#_Toc166157850> ;
    dcat:landingPage "https://www.legislation.gov.au/F2021L00319/2024-04-30/2024-04-30/text/original/epub/OEBPS/document_1/document_1.html#_Toc166157850"^^xsd:anyURI ;
    dcat:theme legcons:Item .

F2021L00319:170 a legcons:Part,
        owl:Class,
        dcat:Resource ;
    rdfs:label "Part - P170 Part 4 Suspension of livestock export licence"@en-AU ;
    dct:isPartOf F2021L00319:125 ;
    dct:isReferencedBy F2021L00319: ;
    rdfs:comment "Part 4 Suspension of livestock export licence - Abrievated Graph Key: P170"@en-AU ;
    skos:definition "Part 4 Suspension of livestock export licence"@en-AU ;
    skos:narrower F2021L00319:125 ;
    skos:prefLabel "Part P170"@en-AU ;
    dcat:accessURL <https://www.legislation.gov.au/F2021L00319/2024-04-30/2024-04-30/text/original/epub/OEBPS/document_1/document_1.html#_Toc166158003> ;
    dcat:landingPage "https://www.legislation.gov.au/F2021L00319/2024-04-30/2024-04-30/text/original/epub/OEBPS/document_1/document_1.html#_Toc166158003"^^xsd:anyURI ;
    dcat:theme legcons:Part .

F2021L00319:171 a legcons:Item,
        owl:Class,
        dcat:Resource ;
    rdfs:label "Item - I171 6 27  Other grounds for suspension"@en-AU ;
    dct:isPartOf F2021L00319:125 ;
    dct:isReferencedBy F2021L00319: ;
    rdfs:comment "6 27  Other grounds for suspension - Abrievated Graph Key: I171"@en-AU ;
    skos:definition "6 27  Other grounds for suspension"@en-AU ;
    skos:narrower F2021L00319:125 ;
    skos:prefLabel "Item I171"@en-AU ;
    dcat:accessURL <https://www.legislation.gov.au/F2021L00319/2024-04-30/2024-04-30/text/original/epub/OEBPS/document_1/document_1.html#_Toc166158004> ;
    dcat:landingPage "https://www.legislation.gov.au/F2021L00319/2024-04-30/2024-04-30/text/original/epub/OEBPS/document_1/document_1.html#_Toc166158004"^^xsd:anyURI ;
    dcat:theme legcons:Item .

F2021L00319:172 a legcons:Part,
        owl:Class,
        dcat:Resource ;
    rdfs:label "Part - P172 Part 5 Revocation of livestock export licence"@en-AU ;
    dct:isPartOf F2021L00319:125 ;
    dct:isReferencedBy F2021L00319: ;
    rdfs:comment "Part 5 Revocation of livestock export licence - Abrievated Graph Key: P172"@en-AU ;
    skos:definition "Part 5 Revocation of livestock export licence"@en-AU ;
    skos:narrower F2021L00319:125 ;
    skos:prefLabel "Part P172"@en-AU ;
    dcat:accessURL <https://www.legislation.gov.au/F2021L00319/2024-04-30/2024-04-30/text/original/epub/OEBPS/document_1/document_1.html#_Toc166158005> ;
    dcat:landingPage "https://www.legislation.gov.au/F2021L00319/2024-04-30/2024-04-30/text/original/epub/OEBPS/document_1/document_1.html#_Toc166158005"^^xsd:anyURI ;
    dcat:theme legcons:Part .

F2021L00319:173 a legcons:Item,
        owl:Class,
        dcat:Resource ;
    rdfs:label "Item - I173 6 28  Other grounds for revocation"@en-AU ;
    dct:isPartOf F2021L00319:125 ;
    dct:isReferencedBy F2021L00319: ;
    rdfs:comment "6 28  Other grounds for revocation - Abrievated Graph Key: I173"@en-AU ;
    skos:definition "6 28  Other grounds for revocation"@en-AU ;
    skos:narrower F2021L00319:125 ;
    skos:prefLabel "Item I173"@en-AU ;
    dcat:accessURL <https://www.legislation.gov.au/F2021L00319/2024-04-30/2024-04-30/text/original/epub/OEBPS/document_1/document_1.html#_Toc166158006> ;
    dcat:landingPage "https://www.legislation.gov.au/F2021L00319/2024-04-30/2024-04-30/text/original/epub/OEBPS/document_1/document_1.html#_Toc166158006"^^xsd:anyURI ;
    dcat:theme legcons:Item .

F2021L00319:174 a legcons:Part,
        owl:Class,
        dcat:Resource ;
    rdfs:label "Part - P174 Part 6 Obligations of holders of livestock export licences"@en-AU ;
    dct:isPartOf F2021L00319:125 ;
    dct:isReferencedBy F2021L00319: ;
    rdfs:comment "Part 6 Obligations of holders of livestock export licences - Abrievated Graph Key: P174"@en-AU ;
    skos:definition "Part 6 Obligations of holders of livestock export licences"@en-AU ;
    skos:narrower F2021L00319:125 ;
    skos:prefLabel "Part P174"@en-AU ;
    dcat:accessURL <https://www.legislation.gov.au/F2021L00319/2024-04-30/2024-04-30/text/original/epub/OEBPS/document_1/document_1.html#_Toc166158007> ;
    dcat:landingPage "https://www.legislation.gov.au/F2021L00319/2024-04-30/2024-04-30/text/original/epub/OEBPS/document_1/document_1.html#_Toc166158007"^^xsd:anyURI ;
    dcat:theme legcons:Part .

F2021L00319:175 a legcons:Item,
        owl:Class,
        dcat:Resource ;
    rdfs:label "Item - I175 6 29  Other events of which Secretary must be notified"@en-AU ;
    dct:isPartOf F2021L00319:125 ;
    dct:isReferencedBy F2021L00319: ;
    rdfs:comment "6 29  Other events of which Secretary must be notified - Abrievated Graph Key: I175"@en-AU ;
    skos:definition "6 29  Other events of which Secretary must be notified"@en-AU ;
    skos:narrower F2021L00319:125 ;
    skos:prefLabel "Item I175"@en-AU ;
    dcat:accessURL <https://www.legislation.gov.au/F2021L00319/2024-04-30/2024-04-30/text/original/epub/OEBPS/document_1/document_1.html#_Toc166158008> ;
    dcat:landingPage "https://www.legislation.gov.au/F2021L00319/2024-04-30/2024-04-30/text/original/epub/OEBPS/document_1/document_1.html#_Toc166158008"^^xsd:anyURI ;
    dcat:theme legcons:Item .

F2021L00319:176 a legcons:Part,
        owl:Class,
        dcat:Resource ;
    rdfs:label "Part - P176 Part 7 Fit and proper persons"@en-AU ;
    dct:isPartOf F2021L00319:125 ;
    dct:isReferencedBy F2021L00319: ;
    rdfs:comment "Part 7 Fit and proper persons - Abrievated Graph Key: P176"@en-AU ;
    skos:definition "Part 7 Fit and proper persons"@en-AU ;
    skos:narrower F2021L00319:125 ;
    skos:prefLabel "Part P176"@en-AU ;
    dcat:accessURL <https://www.legislation.gov.au/F2021L00319/2024-04-30/2024-04-30/text/original/epub/OEBPS/document_1/document_1.html#_Toc166158009> ;
    dcat:landingPage "https://www.legislation.gov.au/F2021L00319/2024-04-30/2024-04-30/text/original/epub/OEBPS/document_1/document_1.html#_Toc166158009"^^xsd:anyURI ;
    dcat:theme legcons:Part .

F2021L00319:177 a legcons:Item,
        owl:Class,
        dcat:Resource ;
    rdfs:label "Item - I177 6 30  Kinds of persons who are required to be fit and proper persons"@en-AU ;
    dct:isPartOf F2021L00319:125 ;
    dct:isReferencedBy F2021L00319: ;
    rdfs:comment "6 30  Kinds of persons who are required to be fit and proper persons - Abrievated Graph Key: I177"@en-AU ;
    skos:definition "6 30  Kinds of persons who are required to be fit and proper persons"@en-AU ;
    skos:narrower F2021L00319:125 ;
    skos:prefLabel "Item I177"@en-AU ;
    dcat:accessURL <https://www.legislation.gov.au/F2021L00319/2024-04-30/2024-04-30/text/original/epub/OEBPS/document_1/document_1.html#_Toc166158010> ;
    dcat:landingPage "https://www.legislation.gov.au/F2021L00319/2024-04-30/2024-04-30/text/original/epub/OEBPS/document_1/document_1.html#_Toc166158010"^^xsd:anyURI ;
    dcat:theme legcons:Item .

F2021L00319:178 a legcons:Part,
        owl:Class,
        dcat:Resource ;
    rdfs:label "Part - P178 Part 8 Matters relating to applications"@en-AU ;
    dct:isPartOf F2021L00319:125 ;
    dct:isReferencedBy F2021L00319: ;
    rdfs:comment "Part 8 Matters relating to applications - Abrievated Graph Key: P178"@en-AU ;
    skos:definition "Part 8 Matters relating to applications"@en-AU ;
    skos:narrower F2021L00319:125 ;
    skos:prefLabel "Part P178"@en-AU ;
    dcat:accessURL <https://www.legislation.gov.au/F2021L00319/2024-04-30/2024-04-30/text/original/epub/OEBPS/document_1/document_1.html#_Toc166158011> ;
    dcat:landingPage "https://www.legislation.gov.au/F2021L00319/2024-04-30/2024-04-30/text/original/epub/OEBPS/document_1/document_1.html#_Toc166158011"^^xsd:anyURI ;
    dcat:theme legcons:Part .

F2021L00319:179 a legcons:Item,
        owl:Class,
        dcat:Resource ;
    rdfs:label "Item - I179 6 31  Application of this Part"@en-AU ;
    dct:isPartOf F2021L00319:125 ;
    dct:isReferencedBy F2021L00319: ;
    rdfs:comment "6 31  Application of this Part - Abrievated Graph Key: I179"@en-AU ;
    skos:definition "6 31  Application of this Part"@en-AU ;
    skos:narrower F2021L00319:125 ;
    skos:prefLabel "Item I179"@en-AU ;
    dcat:accessURL <https://www.legislation.gov.au/F2021L00319/2024-04-30/2024-04-30/text/original/epub/OEBPS/document_1/document_1.html#_Toc166158012> ;
    dcat:landingPage "https://www.legislation.gov.au/F2021L00319/2024-04-30/2024-04-30/text/original/epub/OEBPS/document_1/document_1.html#_Toc166158012"^^xsd:anyURI ;
    dcat:theme legcons:Item .

F2021L00319:18 a legcons:Part,
        owl:Class,
        dcat:Resource ;
    rdfs:label "Part - P18 Part 2 Exemptions"@en-AU ;
    dct:isPartOf F2021L00319:9 ;
    dct:isReferencedBy F2021L00319: ;
    rdfs:comment "Part 2 Exemptions - Abrievated Graph Key: P18"@en-AU ;
    skos:definition "Part 2 Exemptions"@en-AU ;
    skos:narrower F2021L00319:9 ;
    skos:prefLabel "Part P18"@en-AU ;
    dcat:accessURL <https://www.legislation.gov.au/F2021L00319/2024-04-30/2024-04-30/text/original/epub/OEBPS/document_1/document_1.html#_Toc166157851> ;
    dcat:landingPage "https://www.legislation.gov.au/F2021L00319/2024-04-30/2024-04-30/text/original/epub/OEBPS/document_1/document_1.html#_Toc166157851"^^xsd:anyURI ;
    dcat:theme legcons:Part .

F2021L00319:180 a legcons:Item,
        owl:Class,
        dcat:Resource ;
    rdfs:label "Item - I180 6 32  Initial consideration period"@en-AU ;
    dct:isPartOf F2021L00319:125 ;
    dct:isReferencedBy F2021L00319: ;
    rdfs:comment "6 32  Initial consideration period - Abrievated Graph Key: I180"@en-AU ;
    skos:definition "6 32  Initial consideration period"@en-AU ;
    skos:narrower F2021L00319:125 ;
    skos:prefLabel "Item I180"@en-AU ;
    dcat:accessURL <https://www.legislation.gov.au/F2021L00319/2024-04-30/2024-04-30/text/original/epub/OEBPS/document_1/document_1.html#_Toc166158013> ;
    dcat:landingPage "https://www.legislation.gov.au/F2021L00319/2024-04-30/2024-04-30/text/original/epub/OEBPS/document_1/document_1.html#_Toc166158013"^^xsd:anyURI ;
    dcat:theme legcons:Item .

F2021L00319:181 a legcons:Item,
        owl:Class,
        dcat:Resource ;
    rdfs:label "Item - I181 6 33  Maximum period within which request relating to application must be complied with"@en-AU ;
    dct:isPartOf F2021L00319:125 ;
    dct:isReferencedBy F2021L00319: ;
    rdfs:comment "6 33  Maximum period within which request relating to application must be complied with - Abrievated Graph Key: I181"@en-AU ;
    skos:definition "6 33  Maximum period within which request relating to application must be complied with"@en-AU ;
    skos:narrower F2021L00319:125 ;
    skos:prefLabel "Item I181"@en-AU ;
    dcat:accessURL <https://www.legislation.gov.au/F2021L00319/2024-04-30/2024-04-30/text/original/epub/OEBPS/document_1/document_1.html#_Toc166158014> ;
    dcat:landingPage "https://www.legislation.gov.au/F2021L00319/2024-04-30/2024-04-30/text/original/epub/OEBPS/document_1/document_1.html#_Toc166158014"^^xsd:anyURI ;
    dcat:theme legcons:Item .

F2021L00319:182 a legcons:Part,
        owl:Class,
        dcat:Resource ;
    rdfs:label "Part - P182 Part 9 Exporter supply chain assurance systems"@en-AU ;
    dct:isPartOf F2021L00319:125 ;
    dct:isReferencedBy F2021L00319: ;
    rdfs:comment "Part 9 Exporter supply chain assurance systems - Abrievated Graph Key: P182"@en-AU ;
    skos:definition "Part 9 Exporter supply chain assurance systems"@en-AU ;
    skos:narrower F2021L00319:125 ;
    skos:prefLabel "Part P182"@en-AU ;
    dcat:accessURL <https://www.legislation.gov.au/F2021L00319/2024-04-30/2024-04-30/text/original/epub/OEBPS/document_1/document_1.html#_Toc166158015> ;
    dcat:landingPage "https://www.legislation.gov.au/F2021L00319/2024-04-30/2024-04-30/text/original/epub/OEBPS/document_1/document_1.html#_Toc166158015"^^xsd:anyURI ;
    dcat:theme legcons:Part .

F2021L00319:184 a legcons:Item,
        owl:Class,
        dcat:Resource ;
    rdfs:label "Item - I184 6 34  Meaning of ESCAS"@en-AU ;
    dct:isPartOf F2021L00319:183 ;
    dct:isReferencedBy F2021L00319: ;
    rdfs:comment "6 34  Meaning of ESCAS - Abrievated Graph Key: I184"@en-AU ;
    skos:definition "6 34  Meaning of ESCAS"@en-AU ;
    skos:narrower F2021L00319:183 ;
    skos:prefLabel "Item I184"@en-AU ;
    dcat:accessURL <https://www.legislation.gov.au/F2021L00319/2024-04-30/2024-04-30/text/original/epub/OEBPS/document_1/document_1.html#_Toc166158017> ;
    dcat:landingPage "https://www.legislation.gov.au/F2021L00319/2024-04-30/2024-04-30/text/original/epub/OEBPS/document_1/document_1.html#_Toc166158017"^^xsd:anyURI ;
    dcat:theme legcons:Item .

F2021L00319:185 a legcons:Item,
        owl:Class,
        dcat:Resource ;
    rdfs:label "Item - I185 6 35  Holder of livestock export licence may apply for approval of proposed ESCAS"@en-AU ;
    dct:isPartOf F2021L00319:183 ;
    dct:isReferencedBy F2021L00319: ;
    rdfs:comment "6 35  Holder of livestock export licence may apply for approval of proposed ESCAS - Abrievated Graph Key: I185"@en-AU ;
    skos:definition "6 35  Holder of livestock export licence may apply for approval of proposed ESCAS"@en-AU ;
    skos:narrower F2021L00319:183 ;
    skos:prefLabel "Item I185"@en-AU ;
    dcat:accessURL <https://www.legislation.gov.au/F2021L00319/2024-04-30/2024-04-30/text/original/epub/OEBPS/document_1/document_1.html#_Toc166158018> ;
    dcat:landingPage "https://www.legislation.gov.au/F2021L00319/2024-04-30/2024-04-30/text/original/epub/OEBPS/document_1/document_1.html#_Toc166158018"^^xsd:anyURI ;
    dcat:theme legcons:Item .

F2021L00319:186 a legcons:Item,
        owl:Class,
        dcat:Resource ;
    rdfs:label "Item - I186 6 36  Requirements for applications"@en-AU ;
    dct:isPartOf F2021L00319:183 ;
    dct:isReferencedBy F2021L00319: ;
    rdfs:comment "6 36  Requirements for applications - Abrievated Graph Key: I186"@en-AU ;
    skos:definition "6 36  Requirements for applications"@en-AU ;
    skos:narrower F2021L00319:183 ;
    skos:prefLabel "Item I186"@en-AU ;
    dcat:accessURL <https://www.legislation.gov.au/F2021L00319/2024-04-30/2024-04-30/text/original/epub/OEBPS/document_1/document_1.html#_Toc166158019> ;
    dcat:landingPage "https://www.legislation.gov.au/F2021L00319/2024-04-30/2024-04-30/text/original/epub/OEBPS/document_1/document_1.html#_Toc166158019"^^xsd:anyURI ;
    dcat:theme legcons:Item .

F2021L00319:187 a legcons:Item,
        owl:Class,
        dcat:Resource ;
    rdfs:label "Item - I187 6 37  Secretary may approve proposed ESCAS"@en-AU ;
    dct:isPartOf F2021L00319:183 ;
    dct:isReferencedBy F2021L00319: ;
    rdfs:comment "6 37  Secretary may approve proposed ESCAS - Abrievated Graph Key: I187"@en-AU ;
    skos:definition "6 37  Secretary may approve proposed ESCAS"@en-AU ;
    skos:narrower F2021L00319:183 ;
    skos:prefLabel "Item I187"@en-AU ;
    dcat:accessURL <https://www.legislation.gov.au/F2021L00319/2024-04-30/2024-04-30/text/original/epub/OEBPS/document_1/document_1.html#_Toc166158020> ;
    dcat:landingPage "https://www.legislation.gov.au/F2021L00319/2024-04-30/2024-04-30/text/original/epub/OEBPS/document_1/document_1.html#_Toc166158020"^^xsd:anyURI ;
    dcat:theme legcons:Item .

F2021L00319:188 a legcons:Item,
        owl:Class,
        dcat:Resource ;
    rdfs:label "Item - I188 6 38  Period of effect of approved ESCAS"@en-AU ;
    dct:isPartOf F2021L00319:183 ;
    dct:isReferencedBy F2021L00319: ;
    rdfs:comment "6 38  Period of effect of approved ESCAS - Abrievated Graph Key: I188"@en-AU ;
    skos:definition "6 38  Period of effect of approved ESCAS"@en-AU ;
    skos:narrower F2021L00319:183 ;
    skos:prefLabel "Item I188"@en-AU ;
    dcat:accessURL <https://www.legislation.gov.au/F2021L00319/2024-04-30/2024-04-30/text/original/epub/OEBPS/document_1/document_1.html#_Toc166158021> ;
    dcat:landingPage "https://www.legislation.gov.au/F2021L00319/2024-04-30/2024-04-30/text/original/epub/OEBPS/document_1/document_1.html#_Toc166158021"^^xsd:anyURI ;
    dcat:theme legcons:Item .

F2021L00319:19 a legcons:Item,
        owl:Class,
        dcat:Resource ;
    rdfs:label "Item - I19 2 6  Application of this Part"@en-AU ;
    dct:isPartOf F2021L00319:9 ;
    dct:isReferencedBy F2021L00319: ;
    rdfs:comment "2 6  Application of this Part - Abrievated Graph Key: I19"@en-AU ;
    skos:definition "2 6  Application of this Part"@en-AU ;
    skos:narrower F2021L00319:9 ;
    skos:prefLabel "Item I19"@en-AU ;
    dcat:accessURL <https://www.legislation.gov.au/F2021L00319/2024-04-30/2024-04-30/text/original/epub/OEBPS/document_1/document_1.html#_Toc166157852> ;
    dcat:landingPage "https://www.legislation.gov.au/F2021L00319/2024-04-30/2024-04-30/text/original/epub/OEBPS/document_1/document_1.html#_Toc166157852"^^xsd:anyURI ;
    dcat:theme legcons:Item .

F2021L00319:190 a legcons:Item,
        owl:Class,
        dcat:Resource ;
    rdfs:label "Item - I190 6 39  Holder of approved ESCAS may apply to Secretary to vary ESCAS or conditions of ESCAS"@en-AU ;
    dct:isPartOf F2021L00319:189 ;
    dct:isReferencedBy F2021L00319: ;
    rdfs:comment "6 39  Holder of approved ESCAS may apply to Secretary to vary ESCAS or conditions of ESCAS - Abrievated Graph Key: I190"@en-AU ;
    skos:definition "6 39  Holder of approved ESCAS may apply to Secretary to vary ESCAS or conditions of ESCAS"@en-AU ;
    skos:narrower F2021L00319:189 ;
    skos:prefLabel "Item I190"@en-AU ;
    dcat:accessURL <https://www.legislation.gov.au/F2021L00319/2024-04-30/2024-04-30/text/original/epub/OEBPS/document_1/document_1.html#_Toc166158023> ;
    dcat:landingPage "https://www.legislation.gov.au/F2021L00319/2024-04-30/2024-04-30/text/original/epub/OEBPS/document_1/document_1.html#_Toc166158023"^^xsd:anyURI ;
    dcat:theme legcons:Item .

F2021L00319:191 a legcons:Item,
        owl:Class,
        dcat:Resource ;
    rdfs:label "Item - I191 6 40  Secretary may require approved ESCAS to be varied or vary conditions of approved ESCAS"@en-AU ;
    dct:isPartOf F2021L00319:189 ;
    dct:isReferencedBy F2021L00319: ;
    rdfs:comment "6 40  Secretary may require approved ESCAS to be varied or vary conditions of approved ESCAS - Abrievated Graph Key: I191"@en-AU ;
    skos:definition "6 40  Secretary may require approved ESCAS to be varied or vary conditions of approved ESCAS"@en-AU ;
    skos:narrower F2021L00319:189 ;
    skos:prefLabel "Item I191"@en-AU ;
    dcat:accessURL <https://www.legislation.gov.au/F2021L00319/2024-04-30/2024-04-30/text/original/epub/OEBPS/document_1/document_1.html#_Toc166158024> ;
    dcat:landingPage "https://www.legislation.gov.au/F2021L00319/2024-04-30/2024-04-30/text/original/epub/OEBPS/document_1/document_1.html#_Toc166158024"^^xsd:anyURI ;
    dcat:theme legcons:Item .

F2021L00319:192 a legcons:Item,
        owl:Class,
        dcat:Resource ;
    rdfs:label "Item - I192 6 41  Effect of varied approved ESCAS"@en-AU ;
    dct:isPartOf F2021L00319:189 ;
    dct:isReferencedBy F2021L00319: ;
    rdfs:comment "6 41  Effect of varied approved ESCAS - Abrievated Graph Key: I192"@en-AU ;
    skos:definition "6 41  Effect of varied approved ESCAS"@en-AU ;
    skos:narrower F2021L00319:189 ;
    skos:prefLabel "Item I192"@en-AU ;
    dcat:accessURL <https://www.legislation.gov.au/F2021L00319/2024-04-30/2024-04-30/text/original/epub/OEBPS/document_1/document_1.html#_Toc166158025> ;
    dcat:landingPage "https://www.legislation.gov.au/F2021L00319/2024-04-30/2024-04-30/text/original/epub/OEBPS/document_1/document_1.html#_Toc166158025"^^xsd:anyURI ;
    dcat:theme legcons:Item .

F2021L00319:194 a legcons:Item,
        owl:Class,
        dcat:Resource ;
    rdfs:label "Item - I194 6 42  Secretary may revoke approved ESCAS"@en-AU ;
    dct:isPartOf F2021L00319:193 ;
    dct:isReferencedBy F2021L00319: ;
    rdfs:comment "6 42  Secretary may revoke approved ESCAS - Abrievated Graph Key: I194"@en-AU ;
    skos:definition "6 42  Secretary may revoke approved ESCAS"@en-AU ;
    skos:narrower F2021L00319:193 ;
    skos:prefLabel "Item I194"@en-AU ;
    dcat:accessURL <https://www.legislation.gov.au/F2021L00319/2024-04-30/2024-04-30/text/original/epub/OEBPS/document_1/document_1.html#_Toc166158027> ;
    dcat:landingPage "https://www.legislation.gov.au/F2021L00319/2024-04-30/2024-04-30/text/original/epub/OEBPS/document_1/document_1.html#_Toc166158027"^^xsd:anyURI ;
    dcat:theme legcons:Item .

F2021L00319:195 a legcons:Item,
        owl:Class,
        dcat:Resource ;
    rdfs:label "Item - I195 6 42 A  Notice of revocation"@en-AU ;
    dct:isPartOf F2021L00319:193 ;
    dct:isReferencedBy F2021L00319: ;
    rdfs:comment "6 42 A  Notice of revocation - Abrievated Graph Key: I195"@en-AU ;
    skos:definition "6 42 A  Notice of revocation"@en-AU ;
    skos:narrower F2021L00319:193 ;
    skos:prefLabel "Item I195"@en-AU ;
    dcat:accessURL <https://www.legislation.gov.au/F2021L00319/2024-04-30/2024-04-30/text/original/epub/OEBPS/document_1/document_1.html#_Toc166158028> ;
    dcat:landingPage "https://www.legislation.gov.au/F2021L00319/2024-04-30/2024-04-30/text/original/epub/OEBPS/document_1/document_1.html#_Toc166158028"^^xsd:anyURI ;
    dcat:theme legcons:Item .

F2021L00319:197 a legcons:Item,
        owl:Class,
        dcat:Resource ;
    rdfs:label "Item - I197 6 43  Holder of approved ESCAS must notify Secretary of change in circumstance"@en-AU ;
    dct:isPartOf F2021L00319:196 ;
    dct:isReferencedBy F2021L00319: ;
    rdfs:comment "6 43  Holder of approved ESCAS must notify Secretary of change in circumstance - Abrievated Graph Key: I197"@en-AU ;
    skos:definition "6 43  Holder of approved ESCAS must notify Secretary of change in circumstance"@en-AU ;
    skos:narrower F2021L00319:196 ;
    skos:prefLabel "Item I197"@en-AU ;
    dcat:accessURL <https://www.legislation.gov.au/F2021L00319/2024-04-30/2024-04-30/text/original/epub/OEBPS/document_1/document_1.html#_Toc166158030> ;
    dcat:landingPage "https://www.legislation.gov.au/F2021L00319/2024-04-30/2024-04-30/text/original/epub/OEBPS/document_1/document_1.html#_Toc166158030"^^xsd:anyURI ;
    dcat:theme legcons:Item .

F2021L00319:198 a legcons:Part,
        owl:Class,
        dcat:Resource ;
    rdfs:label "Part - P198 Part 10 Miscellaneous"@en-AU ;
    dct:isPartOf F2021L00319:125 ;
    dct:isReferencedBy F2021L00319: ;
    rdfs:comment "Part 10 Miscellaneous - Abrievated Graph Key: P198"@en-AU ;
    skos:definition "Part 10 Miscellaneous"@en-AU ;
    skos:narrower F2021L00319:125 ;
    skos:prefLabel "Part P198"@en-AU ;
    dcat:accessURL <https://www.legislation.gov.au/F2021L00319/2024-04-30/2024-04-30/text/original/epub/OEBPS/document_1/document_1.html#_Toc166158031> ;
    dcat:landingPage "https://www.legislation.gov.au/F2021L00319/2024-04-30/2024-04-30/text/original/epub/OEBPS/document_1/document_1.html#_Toc166158031"^^xsd:anyURI ;
    dcat:theme legcons:Part .

F2021L00319:199 a legcons:Item,
        owl:Class,
        dcat:Resource ;
    rdfs:label "Item - I199 6 44  Secretary may publish information in daily end of voyage or end of journey reports relating to prescribed livestock"@en-AU ;
    dct:isPartOf F2021L00319:125 ;
    dct:isReferencedBy F2021L00319: ;
    rdfs:comment "6 44  Secretary may publish information in daily end of voyage or end of journey reports relating to prescribed livestock - Abrievated Graph Key: I199"@en-AU ;
    skos:definition "6 44  Secretary may publish information in daily end of voyage or end of journey reports relating to prescribed livestock"@en-AU ;
    skos:narrower F2021L00319:125 ;
    skos:prefLabel "Item I199"@en-AU ;
    dcat:accessURL <https://www.legislation.gov.au/F2021L00319/2024-04-30/2024-04-30/text/original/epub/OEBPS/document_1/document_1.html#_Toc166158032> ;
    dcat:landingPage "https://www.legislation.gov.au/F2021L00319/2024-04-30/2024-04-30/text/original/epub/OEBPS/document_1/document_1.html#_Toc166158032"^^xsd:anyURI ;
    dcat:theme legcons:Item .

F2021L00319:2 a legcons:Part,
        owl:Class,
        dcat:Resource ;
    rdfs:label "Part - P2 Part 1 Preliminary"@en-AU ;
    dct:isPartOf F2021L00319:1 ;
    dct:isReferencedBy F2021L00319: ;
    rdfs:comment "Part 1 Preliminary - Abrievated Graph Key: P2"@en-AU ;
    skos:definition "Part 1 Preliminary"@en-AU ;
    skos:narrower F2021L00319:1 ;
    skos:prefLabel "Part P2"@en-AU ;
    dcat:accessURL <https://www.legislation.gov.au/F2021L00319/2024-04-30/2024-04-30/text/original/epub/OEBPS/document_1/document_1.html#_Toc166157835> ;
    dcat:landingPage "https://www.legislation.gov.au/F2021L00319/2024-04-30/2024-04-30/text/original/epub/OEBPS/document_1/document_1.html#_Toc166157835"^^xsd:anyURI ;
    dcat:theme legcons:Part .

F2021L00319:20 a legcons:Item,
        owl:Class,
        dcat:Resource ;
    rdfs:label "Item - I20 2 7  Exports of small numbers of animals in infrequent consignments"@en-AU ;
    dct:isPartOf F2021L00319:9 ;
    dct:isReferencedBy F2021L00319: ;
    rdfs:comment "2 7  Exports of small numbers of animals in infrequent consignments - Abrievated Graph Key: I20"@en-AU ;
    skos:definition "2 7  Exports of small numbers of animals in infrequent consignments"@en-AU ;
    skos:narrower F2021L00319:9 ;
    skos:prefLabel "Item I20"@en-AU ;
    dcat:accessURL <https://www.legislation.gov.au/F2021L00319/2024-04-30/2024-04-30/text/original/epub/OEBPS/document_1/document_1.html#_Toc166157853> ;
    dcat:landingPage "https://www.legislation.gov.au/F2021L00319/2024-04-30/2024-04-30/text/original/epub/OEBPS/document_1/document_1.html#_Toc166157853"^^xsd:anyURI ;
    dcat:theme legcons:Item .

F2021L00319:202 a legcons:Item,
        owl:Class,
        dcat:Resource ;
    rdfs:label "Item - I202 7 1  Other matters to which Secretary may have regard in relation to application for export permit"@en-AU ;
    dct:isPartOf F2021L00319:201 ;
    dct:isReferencedBy F2021L00319: ;
    rdfs:comment "7 1  Other matters to which Secretary may have regard in relation to application for export permit - Abrievated Graph Key: I202"@en-AU ;
    skos:definition "7 1  Other matters to which Secretary may have regard in relation to application for export permit"@en-AU ;
    skos:narrower F2021L00319:201 ;
    skos:prefLabel "Item I202"@en-AU ;
    dcat:accessURL <https://www.legislation.gov.au/F2021L00319/2024-04-30/2024-04-30/text/original/epub/OEBPS/document_1/document_1.html#_Toc166158035> ;
    dcat:landingPage "https://www.legislation.gov.au/F2021L00319/2024-04-30/2024-04-30/text/original/epub/OEBPS/document_1/document_1.html#_Toc166158035"^^xsd:anyURI ;
    dcat:theme legcons:Item .

F2021L00319:203 a legcons:Item,
        owl:Class,
        dcat:Resource ;
    rdfs:label "Item - I203 7 2  Requirements for export permit"@en-AU ;
    dct:isPartOf F2021L00319:201 ;
    dct:isReferencedBy F2021L00319: ;
    rdfs:comment "7 2  Requirements for export permit - Abrievated Graph Key: I203"@en-AU ;
    skos:definition "7 2  Requirements for export permit"@en-AU ;
    skos:narrower F2021L00319:201 ;
    skos:prefLabel "Item I203"@en-AU ;
    dcat:accessURL <https://www.legislation.gov.au/F2021L00319/2024-04-30/2024-04-30/text/original/epub/OEBPS/document_1/document_1.html#_Toc166158036> ;
    dcat:landingPage "https://www.legislation.gov.au/F2021L00319/2024-04-30/2024-04-30/text/original/epub/OEBPS/document_1/document_1.html#_Toc166158036"^^xsd:anyURI ;
    dcat:theme legcons:Item .

F2021L00319:204 a legcons:Item,
        owl:Class,
        dcat:Resource ;
    rdfs:label "Item - I204 7 3  Conditions of export permit"@en-AU ;
    dct:isPartOf F2021L00319:201 ;
    dct:isReferencedBy F2021L00319: ;
    rdfs:comment "7 3  Conditions of export permit - Abrievated Graph Key: I204"@en-AU ;
    skos:definition "7 3  Conditions of export permit"@en-AU ;
    skos:narrower F2021L00319:201 ;
    skos:prefLabel "Item I204"@en-AU ;
    dcat:accessURL <https://www.legislation.gov.au/F2021L00319/2024-04-30/2024-04-30/text/original/epub/OEBPS/document_1/document_1.html#_Toc166158037> ;
    dcat:landingPage "https://www.legislation.gov.au/F2021L00319/2024-04-30/2024-04-30/text/original/epub/OEBPS/document_1/document_1.html#_Toc166158037"^^xsd:anyURI ;
    dcat:theme legcons:Item .

F2021L00319:205 a legcons:Item,
        owl:Class,
        dcat:Resource ;
    rdfs:label "Item - I205 7 4  Period of effect of export permit"@en-AU ;
    dct:isPartOf F2021L00319:201 ;
    dct:isReferencedBy F2021L00319: ;
    rdfs:comment "7 4  Period of effect of export permit - Abrievated Graph Key: I205"@en-AU ;
    skos:definition "7 4  Period of effect of export permit"@en-AU ;
    skos:narrower F2021L00319:201 ;
    skos:prefLabel "Item I205"@en-AU ;
    dcat:accessURL <https://www.legislation.gov.au/F2021L00319/2024-04-30/2024-04-30/text/original/epub/OEBPS/document_1/document_1.html#_Toc166158038> ;
    dcat:landingPage "https://www.legislation.gov.au/F2021L00319/2024-04-30/2024-04-30/text/original/epub/OEBPS/document_1/document_1.html#_Toc166158038"^^xsd:anyURI ;
    dcat:theme legcons:Item .

F2021L00319:207 a legcons:Item,
        owl:Class,
        dcat:Resource ;
    rdfs:label "Item - I207 7 5  Circumstances for varying export permit for prescribed livestock"@en-AU ;
    dct:isPartOf F2021L00319:206 ;
    dct:isReferencedBy F2021L00319: ;
    rdfs:comment "7 5  Circumstances for varying export permit for prescribed livestock - Abrievated Graph Key: I207"@en-AU ;
    skos:definition "7 5  Circumstances for varying export permit for prescribed livestock"@en-AU ;
    skos:narrower F2021L00319:206 ;
    skos:prefLabel "Item I207"@en-AU ;
    dcat:accessURL <https://www.legislation.gov.au/F2021L00319/2024-04-30/2024-04-30/text/original/epub/OEBPS/document_1/document_1.html#_Toc166158040> ;
    dcat:landingPage "https://www.legislation.gov.au/F2021L00319/2024-04-30/2024-04-30/text/original/epub/OEBPS/document_1/document_1.html#_Toc166158040"^^xsd:anyURI ;
    dcat:theme legcons:Item .

F2021L00319:208 a legcons:Item,
        owl:Class,
        dcat:Resource ;
    rdfs:label "Item - I208 7 6  Period of effect of varied export permit"@en-AU ;
    dct:isPartOf F2021L00319:206 ;
    dct:isReferencedBy F2021L00319: ;
    rdfs:comment "7 6  Period of effect of varied export permit - Abrievated Graph Key: I208"@en-AU ;
    skos:definition "7 6  Period of effect of varied export permit"@en-AU ;
    skos:narrower F2021L00319:206 ;
    skos:prefLabel "Item I208"@en-AU ;
    dcat:accessURL <https://www.legislation.gov.au/F2021L00319/2024-04-30/2024-04-30/text/original/epub/OEBPS/document_1/document_1.html#_Toc166158041> ;
    dcat:landingPage "https://www.legislation.gov.au/F2021L00319/2024-04-30/2024-04-30/text/original/epub/OEBPS/document_1/document_1.html#_Toc166158041"^^xsd:anyURI ;
    dcat:theme legcons:Item .

F2021L00319:209 a legcons:Item,
        owl:Class,
        dcat:Resource ;
    rdfs:label "Item - I209 7 7  Circumstances in which export permit may be suspended"@en-AU ;
    dct:isPartOf F2021L00319:206 ;
    dct:isReferencedBy F2021L00319: ;
    rdfs:comment "7 7  Circumstances in which export permit may be suspended - Abrievated Graph Key: I209"@en-AU ;
    skos:definition "7 7  Circumstances in which export permit may be suspended"@en-AU ;
    skos:narrower F2021L00319:206 ;
    skos:prefLabel "Item I209"@en-AU ;
    dcat:accessURL <https://www.legislation.gov.au/F2021L00319/2024-04-30/2024-04-30/text/original/epub/OEBPS/document_1/document_1.html#_Toc166158042> ;
    dcat:landingPage "https://www.legislation.gov.au/F2021L00319/2024-04-30/2024-04-30/text/original/epub/OEBPS/document_1/document_1.html#_Toc166158042"^^xsd:anyURI ;
    dcat:theme legcons:Item .

F2021L00319:21 a legcons:Item,
        owl:Class,
        dcat:Resource ;
    rdfs:label "Item - I21 2 8  Period for making application for exemption"@en-AU ;
    dct:isPartOf F2021L00319:9 ;
    dct:isReferencedBy F2021L00319: ;
    rdfs:comment "2 8  Period for making application for exemption - Abrievated Graph Key: I21"@en-AU ;
    skos:definition "2 8  Period for making application for exemption"@en-AU ;
    skos:narrower F2021L00319:9 ;
    skos:prefLabel "Item I21"@en-AU ;
    dcat:accessURL <https://www.legislation.gov.au/F2021L00319/2024-04-30/2024-04-30/text/original/epub/OEBPS/document_1/document_1.html#_Toc166157854> ;
    dcat:landingPage "https://www.legislation.gov.au/F2021L00319/2024-04-30/2024-04-30/text/original/epub/OEBPS/document_1/document_1.html#_Toc166157854"^^xsd:anyURI ;
    dcat:theme legcons:Item .

F2021L00319:210 a legcons:Item,
        owl:Class,
        dcat:Resource ;
    rdfs:label "Item - I210 7 8  Other circumstances in which export permit may be revoked"@en-AU ;
    dct:isPartOf F2021L00319:206 ;
    dct:isReferencedBy F2021L00319: ;
    rdfs:comment "7 8  Other circumstances in which export permit may be revoked - Abrievated Graph Key: I210"@en-AU ;
    skos:definition "7 8  Other circumstances in which export permit may be revoked"@en-AU ;
    skos:narrower F2021L00319:206 ;
    skos:prefLabel "Item I210"@en-AU ;
    dcat:accessURL <https://www.legislation.gov.au/F2021L00319/2024-04-30/2024-04-30/text/original/epub/OEBPS/document_1/document_1.html#_Toc166158043> ;
    dcat:landingPage "https://www.legislation.gov.au/F2021L00319/2024-04-30/2024-04-30/text/original/epub/OEBPS/document_1/document_1.html#_Toc166158043"^^xsd:anyURI ;
    dcat:theme legcons:Item .

F2021L00319:212 a legcons:Item,
        owl:Class,
        dcat:Resource ;
    rdfs:label "Item - I212 7 9  Changes that require additional or corrected information to be given to the Secretary"@en-AU ;
    dct:isPartOf F2021L00319:211 ;
    dct:isReferencedBy F2021L00319: ;
    rdfs:comment "7 9  Changes that require additional or corrected information to be given to the Secretary - Abrievated Graph Key: I212"@en-AU ;
    skos:definition "7 9  Changes that require additional or corrected information to be given to the Secretary"@en-AU ;
    skos:narrower F2021L00319:211 ;
    skos:prefLabel "Item I212"@en-AU ;
    dcat:accessURL <https://www.legislation.gov.au/F2021L00319/2024-04-30/2024-04-30/text/original/epub/OEBPS/document_1/document_1.html#_Toc166158045> ;
    dcat:landingPage "https://www.legislation.gov.au/F2021L00319/2024-04-30/2024-04-30/text/original/epub/OEBPS/document_1/document_1.html#_Toc166158045"^^xsd:anyURI ;
    dcat:theme legcons:Item .

F2021L00319:213 a legcons:Item,
        owl:Class,
        dcat:Resource ;
    rdfs:label "Item - I213 7 10  Return of export permit"@en-AU ;
    dct:isPartOf F2021L00319:211 ;
    dct:isReferencedBy F2021L00319: ;
    rdfs:comment "7 10  Return of export permit - Abrievated Graph Key: I213"@en-AU ;
    skos:definition "7 10  Return of export permit"@en-AU ;
    skos:narrower F2021L00319:211 ;
    skos:prefLabel "Item I213"@en-AU ;
    dcat:accessURL <https://www.legislation.gov.au/F2021L00319/2024-04-30/2024-04-30/text/original/epub/OEBPS/document_1/document_1.html#_Toc166158046> ;
    dcat:landingPage "https://www.legislation.gov.au/F2021L00319/2024-04-30/2024-04-30/text/original/epub/OEBPS/document_1/document_1.html#_Toc166158046"^^xsd:anyURI ;
    dcat:theme legcons:Item .

F2021L00319:214 a legcons:Item,
        owl:Class,
        dcat:Resource ;
    rdfs:label "Item - I214 7 11  Notification that prescribed livestock prescribed live animals or prescribed animal reproductive material are not to be exported"@en-AU ;
    dct:isPartOf F2021L00319:211 ;
    dct:isReferencedBy F2021L00319: ;
    rdfs:comment "7 11  Notification that prescribed livestock prescribed live animals or prescribed animal reproductive material are not to be exported - Abrievated Graph Key: I214"@en-AU ;
    skos:definition "7 11  Notification that prescribed livestock prescribed live animals or prescribed animal reproductive material are not to be exported"@en-AU ;
    skos:narrower F2021L00319:211 ;
    skos:prefLabel "Item I214"@en-AU ;
    dcat:accessURL <https://www.legislation.gov.au/F2021L00319/2024-04-30/2024-04-30/text/original/epub/OEBPS/document_1/document_1.html#_Toc166158047> ;
    dcat:landingPage "https://www.legislation.gov.au/F2021L00319/2024-04-30/2024-04-30/text/original/epub/OEBPS/document_1/document_1.html#_Toc166158047"^^xsd:anyURI ;
    dcat:theme legcons:Item .

F2021L00319:218 a legcons:Item,
        owl:Class,
        dcat:Resource ;
    rdfs:label "Item - I218 8 1  Person who must give notice of intention to export"@en-AU ;
    dct:isPartOf F2021L00319:217 ;
    dct:isReferencedBy F2021L00319: ;
    rdfs:comment "8 1  Person who must give notice of intention to export - Abrievated Graph Key: I218"@en-AU ;
    skos:definition "8 1  Person who must give notice of intention to export"@en-AU ;
    skos:narrower F2021L00319:217 ;
    skos:prefLabel "Item I218"@en-AU ;
    dcat:accessURL <https://www.legislation.gov.au/F2021L00319/2024-04-30/2024-04-30/text/original/epub/OEBPS/document_1/document_1.html#_Toc166158051> ;
    dcat:landingPage "https://www.legislation.gov.au/F2021L00319/2024-04-30/2024-04-30/text/original/epub/OEBPS/document_1/document_1.html#_Toc166158051"^^xsd:anyURI ;
    dcat:theme legcons:Item .

F2021L00319:219 a legcons:Item,
        owl:Class,
        dcat:Resource ;
    rdfs:label "Item - I219 8 2  Persons to whom notice of intention to export must be given"@en-AU ;
    dct:isPartOf F2021L00319:217 ;
    dct:isReferencedBy F2021L00319: ;
    rdfs:comment "8 2  Persons to whom notice of intention to export must be given - Abrievated Graph Key: I219"@en-AU ;
    skos:definition "8 2  Persons to whom notice of intention to export must be given"@en-AU ;
    skos:narrower F2021L00319:217 ;
    skos:prefLabel "Item I219"@en-AU ;
    dcat:accessURL <https://www.legislation.gov.au/F2021L00319/2024-04-30/2024-04-30/text/original/epub/OEBPS/document_1/document_1.html#_Toc166158052> ;
    dcat:landingPage "https://www.legislation.gov.au/F2021L00319/2024-04-30/2024-04-30/text/original/epub/OEBPS/document_1/document_1.html#_Toc166158052"^^xsd:anyURI ;
    dcat:theme legcons:Item .

F2021L00319:22 a legcons:Item,
        owl:Class,
        dcat:Resource ;
    rdfs:label "Item - I22 2 9  Conditions of exemptionmatters to which Secretary must have regard"@en-AU ;
    dct:isPartOf F2021L00319:9 ;
    dct:isReferencedBy F2021L00319: ;
    rdfs:comment "2 9  Conditions of exemptionmatters to which Secretary must have regard - Abrievated Graph Key: I22"@en-AU ;
    skos:definition "2 9  Conditions of exemptionmatters to which Secretary must have regard"@en-AU ;
    skos:narrower F2021L00319:9 ;
    skos:prefLabel "Item I22"@en-AU ;
    dcat:accessURL <https://www.legislation.gov.au/F2021L00319/2024-04-30/2024-04-30/text/original/epub/OEBPS/document_1/document_1.html#_Toc166157855> ;
    dcat:landingPage "https://www.legislation.gov.au/F2021L00319/2024-04-30/2024-04-30/text/original/epub/OEBPS/document_1/document_1.html#_Toc166157855"^^xsd:anyURI ;
    dcat:theme legcons:Item .

F2021L00319:220 a legcons:Item,
        owl:Class,
        dcat:Resource ;
    rdfs:label "Item - I220 8 3  When notice of intention to export must be given"@en-AU ;
    dct:isPartOf F2021L00319:217 ;
    dct:isReferencedBy F2021L00319: ;
    rdfs:comment "8 3  When notice of intention to export must be given - Abrievated Graph Key: I220"@en-AU ;
    skos:definition "8 3  When notice of intention to export must be given"@en-AU ;
    skos:narrower F2021L00319:217 ;
    skos:prefLabel "Item I220"@en-AU ;
    dcat:accessURL <https://www.legislation.gov.au/F2021L00319/2024-04-30/2024-04-30/text/original/epub/OEBPS/document_1/document_1.html#_Toc166158053> ;
    dcat:landingPage "https://www.legislation.gov.au/F2021L00319/2024-04-30/2024-04-30/text/original/epub/OEBPS/document_1/document_1.html#_Toc166158053"^^xsd:anyURI ;
    dcat:theme legcons:Item .

F2021L00319:221 a legcons:Item,
        owl:Class,
        dcat:Resource ;
    rdfs:label "Item - I221 8 4  Changes requiring additional or corrected information"@en-AU ;
    dct:isPartOf F2021L00319:217 ;
    dct:isReferencedBy F2021L00319: ;
    rdfs:comment "8 4  Changes requiring additional or corrected information - Abrievated Graph Key: I221"@en-AU ;
    skos:definition "8 4  Changes requiring additional or corrected information"@en-AU ;
    skos:narrower F2021L00319:217 ;
    skos:prefLabel "Item I221"@en-AU ;
    dcat:accessURL <https://www.legislation.gov.au/F2021L00319/2024-04-30/2024-04-30/text/original/epub/OEBPS/document_1/document_1.html#_Toc166158054> ;
    dcat:landingPage "https://www.legislation.gov.au/F2021L00319/2024-04-30/2024-04-30/text/original/epub/OEBPS/document_1/document_1.html#_Toc166158054"^^xsd:anyURI ;
    dcat:theme legcons:Item .

F2021L00319:224 a legcons:Item,
        owl:Class,
        dcat:Resource ;
    rdfs:label "Item - I224 8 5  Approval of premises for pre export quarantine or isolation"@en-AU ;
    dct:isPartOf F2021L00319:223 ;
    dct:isReferencedBy F2021L00319: ;
    rdfs:comment "8 5  Approval of premises for pre export quarantine or isolation - Abrievated Graph Key: I224"@en-AU ;
    skos:definition "8 5  Approval of premises for pre export quarantine or isolation"@en-AU ;
    skos:narrower F2021L00319:223 ;
    skos:prefLabel "Item I224"@en-AU ;
    dcat:accessURL <https://www.legislation.gov.au/F2021L00319/2024-04-30/2024-04-30/text/original/epub/OEBPS/document_1/document_1.html#_Toc166158057> ;
    dcat:landingPage "https://www.legislation.gov.au/F2021L00319/2024-04-30/2024-04-30/text/original/epub/OEBPS/document_1/document_1.html#_Toc166158057"^^xsd:anyURI ;
    dcat:theme legcons:Item .

F2021L00319:225 a legcons:Item,
        owl:Class,
        dcat:Resource ;
    rdfs:label "Item - I225 8 6  Approval of notice of intention to export consignment"@en-AU ;
    dct:isPartOf F2021L00319:223 ;
    dct:isReferencedBy F2021L00319: ;
    rdfs:comment "8 6  Approval of notice of intention to export consignment - Abrievated Graph Key: I225"@en-AU ;
    skos:definition "8 6  Approval of notice of intention to export consignment"@en-AU ;
    skos:narrower F2021L00319:223 ;
    skos:prefLabel "Item I225"@en-AU ;
    dcat:accessURL <https://www.legislation.gov.au/F2021L00319/2024-04-30/2024-04-30/text/original/epub/OEBPS/document_1/document_1.html#_Toc166158058> ;
    dcat:landingPage "https://www.legislation.gov.au/F2021L00319/2024-04-30/2024-04-30/text/original/epub/OEBPS/document_1/document_1.html#_Toc166158058"^^xsd:anyURI ;
    dcat:theme legcons:Item .

F2021L00319:226 a legcons:Item,
        owl:Class,
        dcat:Resource ;
    rdfs:label "Item - I226 8 7  Notice of decision relating to approval of notice of intention to export consignment"@en-AU ;
    dct:isPartOf F2021L00319:223 ;
    dct:isReferencedBy F2021L00319: ;
    rdfs:comment "8 7  Notice of decision relating to approval of notice of intention to export consignment - Abrievated Graph Key: I226"@en-AU ;
    skos:definition "8 7  Notice of decision relating to approval of notice of intention to export consignment"@en-AU ;
    skos:narrower F2021L00319:223 ;
    skos:prefLabel "Item I226"@en-AU ;
    dcat:accessURL <https://www.legislation.gov.au/F2021L00319/2024-04-30/2024-04-30/text/original/epub/OEBPS/document_1/document_1.html#_Toc166158059> ;
    dcat:landingPage "https://www.legislation.gov.au/F2021L00319/2024-04-30/2024-04-30/text/original/epub/OEBPS/document_1/document_1.html#_Toc166158059"^^xsd:anyURI ;
    dcat:theme legcons:Item .

F2021L00319:227 a legcons:Item,
        owl:Class,
        dcat:Resource ;
    rdfs:label "Item - I227 8 8  Variation of approved notice of intention to export consignment or conditions of approval"@en-AU ;
    dct:isPartOf F2021L00319:223 ;
    dct:isReferencedBy F2021L00319: ;
    rdfs:comment "8 8  Variation of approved notice of intention to export consignment or conditions of approval - Abrievated Graph Key: I227"@en-AU ;
    skos:definition "8 8  Variation of approved notice of intention to export consignment or conditions of approval"@en-AU ;
    skos:narrower F2021L00319:223 ;
    skos:prefLabel "Item I227"@en-AU ;
    dcat:accessURL <https://www.legislation.gov.au/F2021L00319/2024-04-30/2024-04-30/text/original/epub/OEBPS/document_1/document_1.html#_Toc166158060> ;
    dcat:landingPage "https://www.legislation.gov.au/F2021L00319/2024-04-30/2024-04-30/text/original/epub/OEBPS/document_1/document_1.html#_Toc166158060"^^xsd:anyURI ;
    dcat:theme legcons:Item .

F2021L00319:228 a legcons:Item,
        owl:Class,
        dcat:Resource ;
    rdfs:label "Item - I228 8 9  Secretary may revoke approval of notice of intention to export consignment"@en-AU ;
    dct:isPartOf F2021L00319:223 ;
    dct:isReferencedBy F2021L00319: ;
    rdfs:comment "8 9  Secretary may revoke approval of notice of intention to export consignment - Abrievated Graph Key: I228"@en-AU ;
    skos:definition "8 9  Secretary may revoke approval of notice of intention to export consignment"@en-AU ;
    skos:narrower F2021L00319:223 ;
    skos:prefLabel "Item I228"@en-AU ;
    dcat:accessURL <https://www.legislation.gov.au/F2021L00319/2024-04-30/2024-04-30/text/original/epub/OEBPS/document_1/document_1.html#_Toc166158061> ;
    dcat:landingPage "https://www.legislation.gov.au/F2021L00319/2024-04-30/2024-04-30/text/original/epub/OEBPS/document_1/document_1.html#_Toc166158061"^^xsd:anyURI ;
    dcat:theme legcons:Item .

F2021L00319:23 a legcons:Item,
        owl:Class,
        dcat:Resource ;
    rdfs:label "Item - I23 2 10  Period of effect of exemption"@en-AU ;
    dct:isPartOf F2021L00319:9 ;
    dct:isReferencedBy F2021L00319: ;
    rdfs:comment "2 10  Period of effect of exemption - Abrievated Graph Key: I23"@en-AU ;
    skos:definition "2 10  Period of effect of exemption"@en-AU ;
    skos:narrower F2021L00319:9 ;
    skos:prefLabel "Item I23"@en-AU ;
    dcat:accessURL <https://www.legislation.gov.au/F2021L00319/2024-04-30/2024-04-30/text/original/epub/OEBPS/document_1/document_1.html#_Toc166157856> ;
    dcat:landingPage "https://www.legislation.gov.au/F2021L00319/2024-04-30/2024-04-30/text/original/epub/OEBPS/document_1/document_1.html#_Toc166157856"^^xsd:anyURI ;
    dcat:theme legcons:Item .

F2021L00319:230 a legcons:Item,
        owl:Class,
        dcat:Resource ;
    rdfs:label "Item - I230 8 10  Approval of premises for pre export quarantine or isolation"@en-AU ;
    dct:isPartOf F2021L00319:229 ;
    dct:isReferencedBy F2021L00319: ;
    rdfs:comment "8 10  Approval of premises for pre export quarantine or isolation - Abrievated Graph Key: I230"@en-AU ;
    skos:definition "8 10  Approval of premises for pre export quarantine or isolation"@en-AU ;
    skos:narrower F2021L00319:229 ;
    skos:prefLabel "Item I230"@en-AU ;
    dcat:accessURL <https://www.legislation.gov.au/F2021L00319/2024-04-30/2024-04-30/text/original/epub/OEBPS/document_1/document_1.html#_Toc166158063> ;
    dcat:landingPage "https://www.legislation.gov.au/F2021L00319/2024-04-30/2024-04-30/text/original/epub/OEBPS/document_1/document_1.html#_Toc166158063"^^xsd:anyURI ;
    dcat:theme legcons:Item .

F2021L00319:231 a legcons:Item,
        owl:Class,
        dcat:Resource ;
    rdfs:label "Item - I231 8 11  Approval of notice of intention to export consignment"@en-AU ;
    dct:isPartOf F2021L00319:229 ;
    dct:isReferencedBy F2021L00319: ;
    rdfs:comment "8 11  Approval of notice of intention to export consignment - Abrievated Graph Key: I231"@en-AU ;
    skos:definition "8 11  Approval of notice of intention to export consignment"@en-AU ;
    skos:narrower F2021L00319:229 ;
    skos:prefLabel "Item I231"@en-AU ;
    dcat:accessURL <https://www.legislation.gov.au/F2021L00319/2024-04-30/2024-04-30/text/original/epub/OEBPS/document_1/document_1.html#_Toc166158064> ;
    dcat:landingPage "https://www.legislation.gov.au/F2021L00319/2024-04-30/2024-04-30/text/original/epub/OEBPS/document_1/document_1.html#_Toc166158064"^^xsd:anyURI ;
    dcat:theme legcons:Item .

F2021L00319:232 a legcons:Item,
        owl:Class,
        dcat:Resource ;
    rdfs:label "Item - I232 8 12  Notice of decision relating to approval of notice of intention to export consignment"@en-AU ;
    dct:isPartOf F2021L00319:229 ;
    dct:isReferencedBy F2021L00319: ;
    rdfs:comment "8 12  Notice of decision relating to approval of notice of intention to export consignment - Abrievated Graph Key: I232"@en-AU ;
    skos:definition "8 12  Notice of decision relating to approval of notice of intention to export consignment"@en-AU ;
    skos:narrower F2021L00319:229 ;
    skos:prefLabel "Item I232"@en-AU ;
    dcat:accessURL <https://www.legislation.gov.au/F2021L00319/2024-04-30/2024-04-30/text/original/epub/OEBPS/document_1/document_1.html#_Toc166158065> ;
    dcat:landingPage "https://www.legislation.gov.au/F2021L00319/2024-04-30/2024-04-30/text/original/epub/OEBPS/document_1/document_1.html#_Toc166158065"^^xsd:anyURI ;
    dcat:theme legcons:Item .

F2021L00319:233 a legcons:Item,
        owl:Class,
        dcat:Resource ;
    rdfs:label "Item - I233 8 13  Variation of approved notice of intention to export consignment or conditions of approval"@en-AU ;
    dct:isPartOf F2021L00319:229 ;
    dct:isReferencedBy F2021L00319: ;
    rdfs:comment "8 13  Variation of approved notice of intention to export consignment or conditions of approval - Abrievated Graph Key: I233"@en-AU ;
    skos:definition "8 13  Variation of approved notice of intention to export consignment or conditions of approval"@en-AU ;
    skos:narrower F2021L00319:229 ;
    skos:prefLabel "Item I233"@en-AU ;
    dcat:accessURL <https://www.legislation.gov.au/F2021L00319/2024-04-30/2024-04-30/text/original/epub/OEBPS/document_1/document_1.html#_Toc166158066> ;
    dcat:landingPage "https://www.legislation.gov.au/F2021L00319/2024-04-30/2024-04-30/text/original/epub/OEBPS/document_1/document_1.html#_Toc166158066"^^xsd:anyURI ;
    dcat:theme legcons:Item .

F2021L00319:234 a legcons:Item,
        owl:Class,
        dcat:Resource ;
    rdfs:label "Item - I234 8 14  Secretary may revoke approval of notice of intention to export consignment"@en-AU ;
    dct:isPartOf F2021L00319:229 ;
    dct:isReferencedBy F2021L00319: ;
    rdfs:comment "8 14  Secretary may revoke approval of notice of intention to export consignment - Abrievated Graph Key: I234"@en-AU ;
    skos:definition "8 14  Secretary may revoke approval of notice of intention to export consignment"@en-AU ;
    skos:narrower F2021L00319:229 ;
    skos:prefLabel "Item I234"@en-AU ;
    dcat:accessURL <https://www.legislation.gov.au/F2021L00319/2024-04-30/2024-04-30/text/original/epub/OEBPS/document_1/document_1.html#_Toc166158067> ;
    dcat:landingPage "https://www.legislation.gov.au/F2021L00319/2024-04-30/2024-04-30/text/original/epub/OEBPS/document_1/document_1.html#_Toc166158067"^^xsd:anyURI ;
    dcat:theme legcons:Item .

F2021L00319:237 a legcons:Item,
        owl:Class,
        dcat:Resource ;
    rdfs:label "Item - I237 8 15  Purpose of this Division"@en-AU ;
    dct:isPartOf F2021L00319:236 ;
    dct:isReferencedBy F2021L00319: ;
    rdfs:comment "8 15  Purpose of this Division - Abrievated Graph Key: I237"@en-AU ;
    skos:definition "8 15  Purpose of this Division"@en-AU ;
    skos:narrower F2021L00319:236 ;
    skos:prefLabel "Item I237"@en-AU ;
    dcat:accessURL <https://www.legislation.gov.au/F2021L00319/2024-04-30/2024-04-30/text/original/epub/OEBPS/document_1/document_1.html#_Toc166158070> ;
    dcat:landingPage "https://www.legislation.gov.au/F2021L00319/2024-04-30/2024-04-30/text/original/epub/OEBPS/document_1/document_1.html#_Toc166158070"^^xsd:anyURI ;
    dcat:theme legcons:Item .

F2021L00319:238 a legcons:Item,
        owl:Class,
        dcat:Resource ;
    rdfs:label "Item - I238 8 16  Tolerances for dimensions of official marks"@en-AU ;
    dct:isPartOf F2021L00319:236 ;
    dct:isReferencedBy F2021L00319: ;
    rdfs:comment "8 16  Tolerances for dimensions of official marks - Abrievated Graph Key: I238"@en-AU ;
    skos:definition "8 16  Tolerances for dimensions of official marks"@en-AU ;
    skos:narrower F2021L00319:236 ;
    skos:prefLabel "Item I238"@en-AU ;
    dcat:accessURL <https://www.legislation.gov.au/F2021L00319/2024-04-30/2024-04-30/text/original/epub/OEBPS/document_1/document_1.html#_Toc166158071> ;
    dcat:landingPage "https://www.legislation.gov.au/F2021L00319/2024-04-30/2024-04-30/text/original/epub/OEBPS/document_1/document_1.html#_Toc166158071"^^xsd:anyURI ;
    dcat:theme legcons:Item .

F2021L00319:239 a legcons:Item,
        owl:Class,
        dcat:Resource ;
    rdfs:label "Item - I239 8 17  Official marktamper indicative metal strap seal"@en-AU ;
    dct:isPartOf F2021L00319:236 ;
    dct:isReferencedBy F2021L00319: ;
    rdfs:comment "8 17  Official marktamper indicative metal strap seal - Abrievated Graph Key: I239"@en-AU ;
    skos:definition "8 17  Official marktamper indicative metal strap seal"@en-AU ;
    skos:narrower F2021L00319:236 ;
    skos:prefLabel "Item I239"@en-AU ;
    dcat:accessURL <https://www.legislation.gov.au/F2021L00319/2024-04-30/2024-04-30/text/original/epub/OEBPS/document_1/document_1.html#_Toc166158072> ;
    dcat:landingPage "https://www.legislation.gov.au/F2021L00319/2024-04-30/2024-04-30/text/original/epub/OEBPS/document_1/document_1.html#_Toc166158072"^^xsd:anyURI ;
    dcat:theme legcons:Item .

F2021L00319:24 a legcons:Item,
        owl:Class,
        dcat:Resource ;
    rdfs:label "Item - I24 2 11  Variation of conditions of exemptionmatters to which Secretary must have regard"@en-AU ;
    dct:isPartOf F2021L00319:9 ;
    dct:isReferencedBy F2021L00319: ;
    rdfs:comment "2 11  Variation of conditions of exemptionmatters to which Secretary must have regard - Abrievated Graph Key: I24"@en-AU ;
    skos:definition "2 11  Variation of conditions of exemptionmatters to which Secretary must have regard"@en-AU ;
    skos:narrower F2021L00319:9 ;
    skos:prefLabel "Item I24"@en-AU ;
    dcat:accessURL <https://www.legislation.gov.au/F2021L00319/2024-04-30/2024-04-30/text/original/epub/OEBPS/document_1/document_1.html#_Toc166157857> ;
    dcat:landingPage "https://www.legislation.gov.au/F2021L00319/2024-04-30/2024-04-30/text/original/epub/OEBPS/document_1/document_1.html#_Toc166157857"^^xsd:anyURI ;
    dcat:theme legcons:Item .

F2021L00319:240 a legcons:Item,
        owl:Class,
        dcat:Resource ;
    rdfs:label "Item - I240 8 18  Official markbolt seal"@en-AU ;
    dct:isPartOf F2021L00319:236 ;
    dct:isReferencedBy F2021L00319: ;
    rdfs:comment "8 18  Official markbolt seal - Abrievated Graph Key: I240"@en-AU ;
    skos:definition "8 18  Official markbolt seal"@en-AU ;
    skos:narrower F2021L00319:236 ;
    skos:prefLabel "Item I240"@en-AU ;
    dcat:accessURL <https://www.legislation.gov.au/F2021L00319/2024-04-30/2024-04-30/text/original/epub/OEBPS/document_1/document_1.html#_Toc166158073> ;
    dcat:landingPage "https://www.legislation.gov.au/F2021L00319/2024-04-30/2024-04-30/text/original/epub/OEBPS/document_1/document_1.html#_Toc166158073"^^xsd:anyURI ;
    dcat:theme legcons:Item .

F2021L00319:241 a legcons:Item,
        owl:Class,
        dcat:Resource ;
    rdfs:label "Item - I241 8 19  Official markcarton seal"@en-AU ;
    dct:isPartOf F2021L00319:236 ;
    dct:isReferencedBy F2021L00319: ;
    rdfs:comment "8 19  Official markcarton seal - Abrievated Graph Key: I241"@en-AU ;
    skos:definition "8 19  Official markcarton seal"@en-AU ;
    skos:narrower F2021L00319:236 ;
    skos:prefLabel "Item I241"@en-AU ;
    dcat:accessURL <https://www.legislation.gov.au/F2021L00319/2024-04-30/2024-04-30/text/original/epub/OEBPS/document_1/document_1.html#_Toc166158074> ;
    dcat:landingPage "https://www.legislation.gov.au/F2021L00319/2024-04-30/2024-04-30/text/original/epub/OEBPS/document_1/document_1.html#_Toc166158074"^^xsd:anyURI ;
    dcat:theme legcons:Item .

F2021L00319:242 a legcons:Item,
        owl:Class,
        dcat:Resource ;
    rdfs:label "Item - I242 8 20  Official markAustralian Government"@en-AU ;
    dct:isPartOf F2021L00319:236 ;
    dct:isReferencedBy F2021L00319: ;
    rdfs:comment "8 20  Official markAustralian Government - Abrievated Graph Key: I242"@en-AU ;
    skos:definition "8 20  Official markAustralian Government"@en-AU ;
    skos:narrower F2021L00319:236 ;
    skos:prefLabel "Item I242"@en-AU ;
    dcat:accessURL <https://www.legislation.gov.au/F2021L00319/2024-04-30/2024-04-30/text/original/epub/OEBPS/document_1/document_1.html#_Toc166158075> ;
    dcat:landingPage "https://www.legislation.gov.au/F2021L00319/2024-04-30/2024-04-30/text/original/epub/OEBPS/document_1/document_1.html#_Toc166158075"^^xsd:anyURI ;
    dcat:theme legcons:Item .

F2021L00319:244 a legcons:Item,
        owl:Class,
        dcat:Resource ;
    rdfs:label "Item - I244 8 21  Purpose and application of this Division"@en-AU ;
    dct:isPartOf F2021L00319:243 ;
    dct:isReferencedBy F2021L00319: ;
    rdfs:comment "8 21  Purpose and application of this Division - Abrievated Graph Key: I244"@en-AU ;
    skos:definition "8 21  Purpose and application of this Division"@en-AU ;
    skos:narrower F2021L00319:243 ;
    skos:prefLabel "Item I244"@en-AU ;
    dcat:accessURL <https://www.legislation.gov.au/F2021L00319/2024-04-30/2024-04-30/text/original/epub/OEBPS/document_1/document_1.html#_Toc166158077> ;
    dcat:landingPage "https://www.legislation.gov.au/F2021L00319/2024-04-30/2024-04-30/text/original/epub/OEBPS/document_1/document_1.html#_Toc166158077"^^xsd:anyURI ;
    dcat:theme legcons:Item .

F2021L00319:245 a legcons:Item,
        owl:Class,
        dcat:Resource ;
    rdfs:label "Item - I245 8 22  Meaning of applied"@en-AU ;
    dct:isPartOf F2021L00319:243 ;
    dct:isReferencedBy F2021L00319: ;
    rdfs:comment "8 22  Meaning of applied - Abrievated Graph Key: I245"@en-AU ;
    skos:definition "8 22  Meaning of applied"@en-AU ;
    skos:narrower F2021L00319:243 ;
    skos:prefLabel "Item I245"@en-AU ;
    dcat:accessURL <https://www.legislation.gov.au/F2021L00319/2024-04-30/2024-04-30/text/original/epub/OEBPS/document_1/document_1.html#_Toc166158078> ;
    dcat:landingPage "https://www.legislation.gov.au/F2021L00319/2024-04-30/2024-04-30/text/original/epub/OEBPS/document_1/document_1.html#_Toc166158078"^^xsd:anyURI ;
    dcat:theme legcons:Item .

F2021L00319:246 a legcons:Item,
        owl:Class,
        dcat:Resource ;
    rdfs:label "Item - I246 8 23  Persons who may manufacture official marks for prescribed livestock prescribed live animals or prescribed animal reproductive material"@en-AU ;
    dct:isPartOf F2021L00319:243 ;
    dct:isReferencedBy F2021L00319: ;
    rdfs:comment "8 23  Persons who may manufacture official marks for prescribed livestock prescribed live animals or prescribed animal reproductive material - Abrievated Graph Key: I246"@en-AU ;
    skos:definition "8 23  Persons who may manufacture official marks for prescribed livestock prescribed live animals or prescribed animal reproductive material"@en-AU ;
    skos:narrower F2021L00319:243 ;
    skos:prefLabel "Item I246"@en-AU ;
    dcat:accessURL <https://www.legislation.gov.au/F2021L00319/2024-04-30/2024-04-30/text/original/epub/OEBPS/document_1/document_1.html#_Toc166158079> ;
    dcat:landingPage "https://www.legislation.gov.au/F2021L00319/2024-04-30/2024-04-30/text/original/epub/OEBPS/document_1/document_1.html#_Toc166158079"^^xsd:anyURI ;
    dcat:theme legcons:Item .

F2021L00319:247 a legcons:Item,
        owl:Class,
        dcat:Resource ;
    rdfs:label "Item - I247 8 24  Persons who may possess official marks that have not been applied"@en-AU ;
    dct:isPartOf F2021L00319:243 ;
    dct:isReferencedBy F2021L00319: ;
    rdfs:comment "8 24  Persons who may possess official marks that have not been applied - Abrievated Graph Key: I247"@en-AU ;
    skos:definition "8 24  Persons who may possess official marks that have not been applied"@en-AU ;
    skos:narrower F2021L00319:243 ;
    skos:prefLabel "Item I247"@en-AU ;
    dcat:accessURL <https://www.legislation.gov.au/F2021L00319/2024-04-30/2024-04-30/text/original/epub/OEBPS/document_1/document_1.html#_Toc166158080> ;
    dcat:landingPage "https://www.legislation.gov.au/F2021L00319/2024-04-30/2024-04-30/text/original/epub/OEBPS/document_1/document_1.html#_Toc166158080"^^xsd:anyURI ;
    dcat:theme legcons:Item .

F2021L00319:248 a legcons:Item,
        owl:Class,
        dcat:Resource ;
    rdfs:label "Item - I248 8 25  Persons who may apply official marks to prescribed livestock prescribed live animals or prescribed animal reproductive material"@en-AU ;
    dct:isPartOf F2021L00319:243 ;
    dct:isReferencedBy F2021L00319: ;
    rdfs:comment "8 25  Persons who may apply official marks to prescribed livestock prescribed live animals or prescribed animal reproductive material - Abrievated Graph Key: I248"@en-AU ;
    skos:definition "8 25  Persons who may apply official marks to prescribed livestock prescribed live animals or prescribed animal reproductive material"@en-AU ;
    skos:narrower F2021L00319:243 ;
    skos:prefLabel "Item I248"@en-AU ;
    dcat:accessURL <https://www.legislation.gov.au/F2021L00319/2024-04-30/2024-04-30/text/original/epub/OEBPS/document_1/document_1.html#_Toc166158081> ;
    dcat:landingPage "https://www.legislation.gov.au/F2021L00319/2024-04-30/2024-04-30/text/original/epub/OEBPS/document_1/document_1.html#_Toc166158081"^^xsd:anyURI ;
    dcat:theme legcons:Item .

F2021L00319:249 a legcons:Item,
        owl:Class,
        dcat:Resource ;
    rdfs:label "Item - I249 8 26  Alteration of and interference with official marks"@en-AU ;
    dct:isPartOf F2021L00319:243 ;
    dct:isReferencedBy F2021L00319: ;
    rdfs:comment "8 26  Alteration of and interference with official marks - Abrievated Graph Key: I249"@en-AU ;
    skos:definition "8 26  Alteration of and interference with official marks"@en-AU ;
    skos:narrower F2021L00319:243 ;
    skos:prefLabel "Item I249"@en-AU ;
    dcat:accessURL <https://www.legislation.gov.au/F2021L00319/2024-04-30/2024-04-30/text/original/epub/OEBPS/document_1/document_1.html#_Toc166158082> ;
    dcat:landingPage "https://www.legislation.gov.au/F2021L00319/2024-04-30/2024-04-30/text/original/epub/OEBPS/document_1/document_1.html#_Toc166158082"^^xsd:anyURI ;
    dcat:theme legcons:Item .

F2021L00319:25 a legcons:Item,
        owl:Class,
        dcat:Resource ;
    rdfs:label "Item - I25 2 12  Revocation of exemptionmatter to which Secretary must have regard"@en-AU ;
    dct:isPartOf F2021L00319:9 ;
    dct:isReferencedBy F2021L00319: ;
    rdfs:comment "2 12  Revocation of exemptionmatter to which Secretary must have regard - Abrievated Graph Key: I25"@en-AU ;
    skos:definition "2 12  Revocation of exemptionmatter to which Secretary must have regard"@en-AU ;
    skos:narrower F2021L00319:9 ;
    skos:prefLabel "Item I25"@en-AU ;
    dcat:accessURL <https://www.legislation.gov.au/F2021L00319/2024-04-30/2024-04-30/text/original/epub/OEBPS/document_1/document_1.html#_Toc166157858> ;
    dcat:landingPage "https://www.legislation.gov.au/F2021L00319/2024-04-30/2024-04-30/text/original/epub/OEBPS/document_1/document_1.html#_Toc166157858"^^xsd:anyURI ;
    dcat:theme legcons:Item .

F2021L00319:250 a legcons:Item,
        owl:Class,
        dcat:Resource ;
    rdfs:label "Item - I250 8 27  Official marks must be legible and securely applied"@en-AU ;
    dct:isPartOf F2021L00319:243 ;
    dct:isReferencedBy F2021L00319: ;
    rdfs:comment "8 27  Official marks must be legible and securely applied - Abrievated Graph Key: I250"@en-AU ;
    skos:definition "8 27  Official marks must be legible and securely applied"@en-AU ;
    skos:narrower F2021L00319:243 ;
    skos:prefLabel "Item I250"@en-AU ;
    dcat:accessURL <https://www.legislation.gov.au/F2021L00319/2024-04-30/2024-04-30/text/original/epub/OEBPS/document_1/document_1.html#_Toc166158083> ;
    dcat:landingPage "https://www.legislation.gov.au/F2021L00319/2024-04-30/2024-04-30/text/original/epub/OEBPS/document_1/document_1.html#_Toc166158083"^^xsd:anyURI ;
    dcat:theme legcons:Item .

F2021L00319:251 a legcons:Item,
        owl:Class,
        dcat:Resource ;
    rdfs:label "Item - I251 8 28  Security of official marks"@en-AU ;
    dct:isPartOf F2021L00319:243 ;
    dct:isReferencedBy F2021L00319: ;
    rdfs:comment "8 28  Security of official marks - Abrievated Graph Key: I251"@en-AU ;
    skos:definition "8 28  Security of official marks"@en-AU ;
    skos:narrower F2021L00319:243 ;
    skos:prefLabel "Item I251"@en-AU ;
    dcat:accessURL <https://www.legislation.gov.au/F2021L00319/2024-04-30/2024-04-30/text/original/epub/OEBPS/document_1/document_1.html#_Toc166158084> ;
    dcat:landingPage "https://www.legislation.gov.au/F2021L00319/2024-04-30/2024-04-30/text/original/epub/OEBPS/document_1/document_1.html#_Toc166158084"^^xsd:anyURI ;
    dcat:theme legcons:Item .

F2021L00319:252 a legcons:Item,
        owl:Class,
        dcat:Resource ;
    rdfs:label "Item - I252 8 29  Removal or defacement of official marks"@en-AU ;
    dct:isPartOf F2021L00319:243 ;
    dct:isReferencedBy F2021L00319: ;
    rdfs:comment "8 29  Removal or defacement of official marks - Abrievated Graph Key: I252"@en-AU ;
    skos:definition "8 29  Removal or defacement of official marks"@en-AU ;
    skos:narrower F2021L00319:243 ;
    skos:prefLabel "Item I252"@en-AU ;
    dcat:accessURL <https://www.legislation.gov.au/F2021L00319/2024-04-30/2024-04-30/text/original/epub/OEBPS/document_1/document_1.html#_Toc166158085> ;
    dcat:landingPage "https://www.legislation.gov.au/F2021L00319/2024-04-30/2024-04-30/text/original/epub/OEBPS/document_1/document_1.html#_Toc166158085"^^xsd:anyURI ;
    dcat:theme legcons:Item .

F2021L00319:253 a legcons:Item,
        owl:Class,
        dcat:Resource ;
    rdfs:label "Item - I253 8 30  Records of official marks manufactured"@en-AU ;
    dct:isPartOf F2021L00319:243 ;
    dct:isReferencedBy F2021L00319: ;
    rdfs:comment "8 30  Records of official marks manufactured - Abrievated Graph Key: I253"@en-AU ;
    skos:definition "8 30  Records of official marks manufactured"@en-AU ;
    skos:narrower F2021L00319:243 ;
    skos:prefLabel "Item I253"@en-AU ;
    dcat:accessURL <https://www.legislation.gov.au/F2021L00319/2024-04-30/2024-04-30/text/original/epub/OEBPS/document_1/document_1.html#_Toc166158086> ;
    dcat:landingPage "https://www.legislation.gov.au/F2021L00319/2024-04-30/2024-04-30/text/original/epub/OEBPS/document_1/document_1.html#_Toc166158086"^^xsd:anyURI ;
    dcat:theme legcons:Item .

F2021L00319:254 a legcons:Item,
        owl:Class,
        dcat:Resource ;
    rdfs:label "Item - I254 8 31  Records of official marks applied removed defaced destroyed or returned"@en-AU ;
    dct:isPartOf F2021L00319:243 ;
    dct:isReferencedBy F2021L00319: ;
    rdfs:comment "8 31  Records of official marks applied removed defaced destroyed or returned - Abrievated Graph Key: I254"@en-AU ;
    skos:definition "8 31  Records of official marks applied removed defaced destroyed or returned"@en-AU ;
    skos:narrower F2021L00319:243 ;
    skos:prefLabel "Item I254"@en-AU ;
    dcat:accessURL <https://www.legislation.gov.au/F2021L00319/2024-04-30/2024-04-30/text/original/epub/OEBPS/document_1/document_1.html#_Toc166158087> ;
    dcat:landingPage "https://www.legislation.gov.au/F2021L00319/2024-04-30/2024-04-30/text/original/epub/OEBPS/document_1/document_1.html#_Toc166158087"^^xsd:anyURI ;
    dcat:theme legcons:Item .

F2021L00319:256 a legcons:Item,
        owl:Class,
        dcat:Resource ;
    rdfs:label "Item - I256 8 32  Purpose of this Division"@en-AU ;
    dct:isPartOf F2021L00319:255 ;
    dct:isReferencedBy F2021L00319: ;
    rdfs:comment "8 32  Purpose of this Division - Abrievated Graph Key: I256"@en-AU ;
    skos:definition "8 32  Purpose of this Division"@en-AU ;
    skos:narrower F2021L00319:255 ;
    skos:prefLabel "Item I256"@en-AU ;
    dcat:accessURL <https://www.legislation.gov.au/F2021L00319/2024-04-30/2024-04-30/text/original/epub/OEBPS/document_1/document_1.html#_Toc166158089> ;
    dcat:landingPage "https://www.legislation.gov.au/F2021L00319/2024-04-30/2024-04-30/text/original/epub/OEBPS/document_1/document_1.html#_Toc166158089"^^xsd:anyURI ;
    dcat:theme legcons:Item .

F2021L00319:257 a legcons:Item,
        owl:Class,
        dcat:Resource ;
    rdfs:label "Item - I257 8 33  Persons who may manufacture or possess official marking devices"@en-AU ;
    dct:isPartOf F2021L00319:255 ;
    dct:isReferencedBy F2021L00319: ;
    rdfs:comment "8 33  Persons who may manufacture or possess official marking devices - Abrievated Graph Key: I257"@en-AU ;
    skos:definition "8 33  Persons who may manufacture or possess official marking devices"@en-AU ;
    skos:narrower F2021L00319:255 ;
    skos:prefLabel "Item I257"@en-AU ;
    dcat:accessURL <https://www.legislation.gov.au/F2021L00319/2024-04-30/2024-04-30/text/original/epub/OEBPS/document_1/document_1.html#_Toc166158090> ;
    dcat:landingPage "https://www.legislation.gov.au/F2021L00319/2024-04-30/2024-04-30/text/original/epub/OEBPS/document_1/document_1.html#_Toc166158090"^^xsd:anyURI ;
    dcat:theme legcons:Item .

F2021L00319:258 a legcons:Item,
        owl:Class,
        dcat:Resource ;
    rdfs:label "Item - I258 8 34  Security of official marking devices"@en-AU ;
    dct:isPartOf F2021L00319:255 ;
    dct:isReferencedBy F2021L00319: ;
    rdfs:comment "8 34  Security of official marking devices - Abrievated Graph Key: I258"@en-AU ;
    skos:definition "8 34  Security of official marking devices"@en-AU ;
    skos:narrower F2021L00319:255 ;
    skos:prefLabel "Item I258"@en-AU ;
    dcat:accessURL <https://www.legislation.gov.au/F2021L00319/2024-04-30/2024-04-30/text/original/epub/OEBPS/document_1/document_1.html#_Toc166158091> ;
    dcat:landingPage "https://www.legislation.gov.au/F2021L00319/2024-04-30/2024-04-30/text/original/epub/OEBPS/document_1/document_1.html#_Toc166158091"^^xsd:anyURI ;
    dcat:theme legcons:Item .

F2021L00319:259 a legcons:Item,
        owl:Class,
        dcat:Resource ;
    rdfs:label "Item - I259 8 35  Damaged or destroyed official marking devices"@en-AU ;
    dct:isPartOf F2021L00319:255 ;
    dct:isReferencedBy F2021L00319: ;
    rdfs:comment "8 35  Damaged or destroyed official marking devices - Abrievated Graph Key: I259"@en-AU ;
    skos:definition "8 35  Damaged or destroyed official marking devices"@en-AU ;
    skos:narrower F2021L00319:255 ;
    skos:prefLabel "Item I259"@en-AU ;
    dcat:accessURL <https://www.legislation.gov.au/F2021L00319/2024-04-30/2024-04-30/text/original/epub/OEBPS/document_1/document_1.html#_Toc166158092> ;
    dcat:landingPage "https://www.legislation.gov.au/F2021L00319/2024-04-30/2024-04-30/text/original/epub/OEBPS/document_1/document_1.html#_Toc166158092"^^xsd:anyURI ;
    dcat:theme legcons:Item .

F2021L00319:26 a legcons:Part,
        owl:Class,
        dcat:Resource ;
    rdfs:label "Part - P26 Part 3 Government certificates"@en-AU ;
    dct:isPartOf F2021L00319:9 ;
    dct:isReferencedBy F2021L00319: ;
    rdfs:comment "Part 3 Government certificates - Abrievated Graph Key: P26"@en-AU ;
    skos:definition "Part 3 Government certificates"@en-AU ;
    skos:narrower F2021L00319:9 ;
    skos:prefLabel "Part P26"@en-AU ;
    dcat:accessURL <https://www.legislation.gov.au/F2021L00319/2024-04-30/2024-04-30/text/original/epub/OEBPS/document_1/document_1.html#_Toc166157859> ;
    dcat:landingPage "https://www.legislation.gov.au/F2021L00319/2024-04-30/2024-04-30/text/original/epub/OEBPS/document_1/document_1.html#_Toc166157859"^^xsd:anyURI ;
    dcat:theme legcons:Part .

F2021L00319:260 a legcons:Item,
        owl:Class,
        dcat:Resource ;
    rdfs:label "Item - I260 8 36  Records of official marking devices manufactured"@en-AU ;
    dct:isPartOf F2021L00319:255 ;
    dct:isReferencedBy F2021L00319: ;
    rdfs:comment "8 36  Records of official marking devices manufactured - Abrievated Graph Key: I260"@en-AU ;
    skos:definition "8 36  Records of official marking devices manufactured"@en-AU ;
    skos:narrower F2021L00319:255 ;
    skos:prefLabel "Item I260"@en-AU ;
    dcat:accessURL <https://www.legislation.gov.au/F2021L00319/2024-04-30/2024-04-30/text/original/epub/OEBPS/document_1/document_1.html#_Toc166158093> ;
    dcat:landingPage "https://www.legislation.gov.au/F2021L00319/2024-04-30/2024-04-30/text/original/epub/OEBPS/document_1/document_1.html#_Toc166158093"^^xsd:anyURI ;
    dcat:theme legcons:Item .

F2021L00319:261 a legcons:Item,
        owl:Class,
        dcat:Resource ;
    rdfs:label "Item - I261 8 37  Records of official marking devices used destroyed or returned"@en-AU ;
    dct:isPartOf F2021L00319:255 ;
    dct:isReferencedBy F2021L00319: ;
    rdfs:comment "8 37  Records of official marking devices used destroyed or returned - Abrievated Graph Key: I261"@en-AU ;
    skos:definition "8 37  Records of official marking devices used destroyed or returned"@en-AU ;
    skos:narrower F2021L00319:255 ;
    skos:prefLabel "Item I261"@en-AU ;
    dcat:accessURL <https://www.legislation.gov.au/F2021L00319/2024-04-30/2024-04-30/text/original/epub/OEBPS/document_1/document_1.html#_Toc166158094> ;
    dcat:landingPage "https://www.legislation.gov.au/F2021L00319/2024-04-30/2024-04-30/text/original/epub/OEBPS/document_1/document_1.html#_Toc166158094"^^xsd:anyURI ;
    dcat:theme legcons:Item .

F2021L00319:265 a legcons:Item,
        owl:Class,
        dcat:Resource ;
    rdfs:label "Item - I265 9 1  References to audit in this Part"@en-AU ;
    dct:isPartOf F2021L00319:264 ;
    dct:isReferencedBy F2021L00319: ;
    rdfs:comment "9 1  References to audit in this Part - Abrievated Graph Key: I265"@en-AU ;
    skos:definition "9 1  References to audit in this Part"@en-AU ;
    skos:narrower F2021L00319:264 ;
    skos:prefLabel "Item I265"@en-AU ;
    dcat:accessURL <https://www.legislation.gov.au/F2021L00319/2024-04-30/2024-04-30/text/original/epub/OEBPS/document_1/document_1.html#_Toc166158098> ;
    dcat:landingPage "https://www.legislation.gov.au/F2021L00319/2024-04-30/2024-04-30/text/original/epub/OEBPS/document_1/document_1.html#_Toc166158098"^^xsd:anyURI ;
    dcat:theme legcons:Item .

F2021L00319:267 a legcons:Item,
        owl:Class,
        dcat:Resource ;
    rdfs:label "Item - I267 9 2  Purpose of this Division"@en-AU ;
    dct:isPartOf F2021L00319:266 ;
    dct:isReferencedBy F2021L00319: ;
    rdfs:comment "9 2  Purpose of this Division - Abrievated Graph Key: I267"@en-AU ;
    skos:definition "9 2  Purpose of this Division"@en-AU ;
    skos:narrower F2021L00319:266 ;
    skos:prefLabel "Item I267"@en-AU ;
    dcat:accessURL <https://www.legislation.gov.au/F2021L00319/2024-04-30/2024-04-30/text/original/epub/OEBPS/document_1/document_1.html#_Toc166158100> ;
    dcat:landingPage "https://www.legislation.gov.au/F2021L00319/2024-04-30/2024-04-30/text/original/epub/OEBPS/document_1/document_1.html#_Toc166158100"^^xsd:anyURI ;
    dcat:theme legcons:Item .

F2021L00319:268 a legcons:Item,
        owl:Class,
        dcat:Resource ;
    rdfs:label "Item - I268 9 3  Manner in which audit must be conducted"@en-AU ;
    dct:isPartOf F2021L00319:266 ;
    dct:isReferencedBy F2021L00319: ;
    rdfs:comment "9 3  Manner in which audit must be conducted - Abrievated Graph Key: I268"@en-AU ;
    skos:definition "9 3  Manner in which audit must be conducted"@en-AU ;
    skos:narrower F2021L00319:266 ;
    skos:prefLabel "Item I268"@en-AU ;
    dcat:accessURL <https://www.legislation.gov.au/F2021L00319/2024-04-30/2024-04-30/text/original/epub/OEBPS/document_1/document_1.html#_Toc166158101> ;
    dcat:landingPage "https://www.legislation.gov.au/F2021L00319/2024-04-30/2024-04-30/text/original/epub/OEBPS/document_1/document_1.html#_Toc166158101"^^xsd:anyURI ;
    dcat:theme legcons:Item .

F2021L00319:269 a legcons:Item,
        owl:Class,
        dcat:Resource ;
    rdfs:label "Item - I269 9 4  Notice of non compliance with requirements"@en-AU ;
    dct:isPartOf F2021L00319:266 ;
    dct:isReferencedBy F2021L00319: ;
    rdfs:comment "9 4  Notice of non compliance with requirements - Abrievated Graph Key: I269"@en-AU ;
    skos:definition "9 4  Notice of non compliance with requirements"@en-AU ;
    skos:narrower F2021L00319:266 ;
    skos:prefLabel "Item I269"@en-AU ;
    dcat:accessURL <https://www.legislation.gov.au/F2021L00319/2024-04-30/2024-04-30/text/original/epub/OEBPS/document_1/document_1.html#_Toc166158102> ;
    dcat:landingPage "https://www.legislation.gov.au/F2021L00319/2024-04-30/2024-04-30/text/original/epub/OEBPS/document_1/document_1.html#_Toc166158102"^^xsd:anyURI ;
    dcat:theme legcons:Item .

F2021L00319:270 a legcons:Item,
        owl:Class,
        dcat:Resource ;
    rdfs:label "Item - I270 9 5  Audit reports"@en-AU ;
    dct:isPartOf F2021L00319:266 ;
    dct:isReferencedBy F2021L00319: ;
    rdfs:comment "9 5  Audit reports - Abrievated Graph Key: I270"@en-AU ;
    skos:definition "9 5  Audit reports"@en-AU ;
    skos:narrower F2021L00319:266 ;
    skos:prefLabel "Item I270"@en-AU ;
    dcat:accessURL <https://www.legislation.gov.au/F2021L00319/2024-04-30/2024-04-30/text/original/epub/OEBPS/document_1/document_1.html#_Toc166158103> ;
    dcat:landingPage "https://www.legislation.gov.au/F2021L00319/2024-04-30/2024-04-30/text/original/epub/OEBPS/document_1/document_1.html#_Toc166158103"^^xsd:anyURI ;
    dcat:theme legcons:Item .

F2021L00319:273 a legcons:Item,
        owl:Class,
        dcat:Resource ;
    rdfs:label "Item - I273 9 6  References to assessment in this Part"@en-AU ;
    dct:isPartOf F2021L00319:272 ;
    dct:isReferencedBy F2021L00319: ;
    rdfs:comment "9 6  References to assessment in this Part - Abrievated Graph Key: I273"@en-AU ;
    skos:definition "9 6  References to assessment in this Part"@en-AU ;
    skos:narrower F2021L00319:272 ;
    skos:prefLabel "Item I273"@en-AU ;
    dcat:accessURL <https://www.legislation.gov.au/F2021L00319/2024-04-30/2024-04-30/text/original/epub/OEBPS/document_1/document_1.html#_Toc166158106> ;
    dcat:landingPage "https://www.legislation.gov.au/F2021L00319/2024-04-30/2024-04-30/text/original/epub/OEBPS/document_1/document_1.html#_Toc166158106"^^xsd:anyURI ;
    dcat:theme legcons:Item .

F2021L00319:275 a legcons:Item,
        owl:Class,
        dcat:Resource ;
    rdfs:label "Item - I275 9 7  Circumstances in which assessment may be required or permitted"@en-AU ;
    dct:isPartOf F2021L00319:274 ;
    dct:isReferencedBy F2021L00319: ;
    rdfs:comment "9 7  Circumstances in which assessment may be required or permitted - Abrievated Graph Key: I275"@en-AU ;
    skos:definition "9 7  Circumstances in which assessment may be required or permitted"@en-AU ;
    skos:narrower F2021L00319:274 ;
    skos:prefLabel "Item I275"@en-AU ;
    dcat:accessURL <https://www.legislation.gov.au/F2021L00319/2024-04-30/2024-04-30/text/original/epub/OEBPS/document_1/document_1.html#_Toc166158108> ;
    dcat:landingPage "https://www.legislation.gov.au/F2021L00319/2024-04-30/2024-04-30/text/original/epub/OEBPS/document_1/document_1.html#_Toc166158108"^^xsd:anyURI ;
    dcat:theme legcons:Item .

F2021L00319:276 a legcons:Item,
        owl:Class,
        dcat:Resource ;
    rdfs:label "Item - I276 9 8  Process to be followed after assessment completed"@en-AU ;
    dct:isPartOf F2021L00319:274 ;
    dct:isReferencedBy F2021L00319: ;
    rdfs:comment "9 8  Process to be followed after assessment completed - Abrievated Graph Key: I276"@en-AU ;
    skos:definition "9 8  Process to be followed after assessment completed"@en-AU ;
    skos:narrower F2021L00319:274 ;
    skos:prefLabel "Item I276"@en-AU ;
    dcat:accessURL <https://www.legislation.gov.au/F2021L00319/2024-04-30/2024-04-30/text/original/epub/OEBPS/document_1/document_1.html#_Toc166158109> ;
    dcat:landingPage "https://www.legislation.gov.au/F2021L00319/2024-04-30/2024-04-30/text/original/epub/OEBPS/document_1/document_1.html#_Toc166158109"^^xsd:anyURI ;
    dcat:theme legcons:Item .

F2021L00319:279 a legcons:Item,
        owl:Class,
        dcat:Resource ;
    rdfs:label "Item - I279 9 9  Purpose of this Part"@en-AU ;
    dct:isPartOf F2021L00319:278 ;
    dct:isReferencedBy F2021L00319: ;
    rdfs:comment "9 9  Purpose of this Part - Abrievated Graph Key: I279"@en-AU ;
    skos:definition "9 9  Purpose of this Part"@en-AU ;
    skos:narrower F2021L00319:278 ;
    skos:prefLabel "Item I279"@en-AU ;
    dcat:accessURL <https://www.legislation.gov.au/F2021L00319/2024-04-30/2024-04-30/text/original/epub/OEBPS/document_1/document_1.html#_Toc166158112> ;
    dcat:landingPage "https://www.legislation.gov.au/F2021L00319/2024-04-30/2024-04-30/text/original/epub/OEBPS/document_1/document_1.html#_Toc166158112"^^xsd:anyURI ;
    dcat:theme legcons:Item .

F2021L00319:28 a legcons:Item,
        owl:Class,
        dcat:Resource ;
    rdfs:label "Item - I28 2 13  Application of this Division"@en-AU ;
    dct:isPartOf F2021L00319:27 ;
    dct:isReferencedBy F2021L00319: ;
    rdfs:comment "2 13  Application of this Division - Abrievated Graph Key: I28"@en-AU ;
    skos:definition "2 13  Application of this Division"@en-AU ;
    skos:narrower F2021L00319:27 ;
    skos:prefLabel "Item I28"@en-AU ;
    dcat:accessURL <https://www.legislation.gov.au/F2021L00319/2024-04-30/2024-04-30/text/original/epub/OEBPS/document_1/document_1.html#_Toc166157861> ;
    dcat:landingPage "https://www.legislation.gov.au/F2021L00319/2024-04-30/2024-04-30/text/original/epub/OEBPS/document_1/document_1.html#_Toc166157861"^^xsd:anyURI ;
    dcat:theme legcons:Item .

F2021L00319:281 a legcons:Item,
        owl:Class,
        dcat:Resource ;
    rdfs:label "Item - I281 9 10  Requirements for accreditation"@en-AU ;
    dct:isPartOf F2021L00319:280 ;
    dct:isReferencedBy F2021L00319: ;
    rdfs:comment "9 10  Requirements for accreditation - Abrievated Graph Key: I281"@en-AU ;
    skos:definition "9 10  Requirements for accreditation"@en-AU ;
    skos:narrower F2021L00319:280 ;
    skos:prefLabel "Item I281"@en-AU ;
    dcat:accessURL <https://www.legislation.gov.au/F2021L00319/2024-04-30/2024-04-30/text/original/epub/OEBPS/document_1/document_1.html#_Toc166158114> ;
    dcat:landingPage "https://www.legislation.gov.au/F2021L00319/2024-04-30/2024-04-30/text/original/epub/OEBPS/document_1/document_1.html#_Toc166158114"^^xsd:anyURI ;
    dcat:theme legcons:Item .

F2021L00319:282 a legcons:Item,
        owl:Class,
        dcat:Resource ;
    rdfs:label "Item - I282 9 11  Application for accreditation"@en-AU ;
    dct:isPartOf F2021L00319:280 ;
    dct:isReferencedBy F2021L00319: ;
    rdfs:comment "9 11  Application for accreditation - Abrievated Graph Key: I282"@en-AU ;
    skos:definition "9 11  Application for accreditation"@en-AU ;
    skos:narrower F2021L00319:280 ;
    skos:prefLabel "Item I282"@en-AU ;
    dcat:accessURL <https://www.legislation.gov.au/F2021L00319/2024-04-30/2024-04-30/text/original/epub/OEBPS/document_1/document_1.html#_Toc166158115> ;
    dcat:landingPage "https://www.legislation.gov.au/F2021L00319/2024-04-30/2024-04-30/text/original/epub/OEBPS/document_1/document_1.html#_Toc166158115"^^xsd:anyURI ;
    dcat:theme legcons:Item .

F2021L00319:283 a legcons:Item,
        owl:Class,
        dcat:Resource ;
    rdfs:label "Item - I283 9 12  Secretary must decide whether to accredit veterinarian"@en-AU ;
    dct:isPartOf F2021L00319:280 ;
    dct:isReferencedBy F2021L00319: ;
    rdfs:comment "9 12  Secretary must decide whether to accredit veterinarian - Abrievated Graph Key: I283"@en-AU ;
    skos:definition "9 12  Secretary must decide whether to accredit veterinarian"@en-AU ;
    skos:narrower F2021L00319:280 ;
    skos:prefLabel "Item I283"@en-AU ;
    dcat:accessURL <https://www.legislation.gov.au/F2021L00319/2024-04-30/2024-04-30/text/original/epub/OEBPS/document_1/document_1.html#_Toc166158116> ;
    dcat:landingPage "https://www.legislation.gov.au/F2021L00319/2024-04-30/2024-04-30/text/original/epub/OEBPS/document_1/document_1.html#_Toc166158116"^^xsd:anyURI ;
    dcat:theme legcons:Item .

F2021L00319:284 a legcons:Item,
        owl:Class,
        dcat:Resource ;
    rdfs:label "Item - I284 9 13  Conditions of accreditation"@en-AU ;
    dct:isPartOf F2021L00319:280 ;
    dct:isReferencedBy F2021L00319: ;
    rdfs:comment "9 13  Conditions of accreditation - Abrievated Graph Key: I284"@en-AU ;
    skos:definition "9 13  Conditions of accreditation"@en-AU ;
    skos:narrower F2021L00319:280 ;
    skos:prefLabel "Item I284"@en-AU ;
    dcat:accessURL <https://www.legislation.gov.au/F2021L00319/2024-04-30/2024-04-30/text/original/epub/OEBPS/document_1/document_1.html#_Toc166158117> ;
    dcat:landingPage "https://www.legislation.gov.au/F2021L00319/2024-04-30/2024-04-30/text/original/epub/OEBPS/document_1/document_1.html#_Toc166158117"^^xsd:anyURI ;
    dcat:theme legcons:Item .

F2021L00319:285 a legcons:Item,
        owl:Class,
        dcat:Resource ;
    rdfs:label "Item - I285 9 14  Notice of accreditation"@en-AU ;
    dct:isPartOf F2021L00319:280 ;
    dct:isReferencedBy F2021L00319: ;
    rdfs:comment "9 14  Notice of accreditation - Abrievated Graph Key: I285"@en-AU ;
    skos:definition "9 14  Notice of accreditation"@en-AU ;
    skos:narrower F2021L00319:280 ;
    skos:prefLabel "Item I285"@en-AU ;
    dcat:accessURL <https://www.legislation.gov.au/F2021L00319/2024-04-30/2024-04-30/text/original/epub/OEBPS/document_1/document_1.html#_Toc166158118> ;
    dcat:landingPage "https://www.legislation.gov.au/F2021L00319/2024-04-30/2024-04-30/text/original/epub/OEBPS/document_1/document_1.html#_Toc166158118"^^xsd:anyURI ;
    dcat:theme legcons:Item .

F2021L00319:286 a legcons:Item,
        owl:Class,
        dcat:Resource ;
    rdfs:label "Item - I286 9 15  Period of effect of accreditation"@en-AU ;
    dct:isPartOf F2021L00319:280 ;
    dct:isReferencedBy F2021L00319: ;
    rdfs:comment "9 15  Period of effect of accreditation - Abrievated Graph Key: I286"@en-AU ;
    skos:definition "9 15  Period of effect of accreditation"@en-AU ;
    skos:narrower F2021L00319:280 ;
    skos:prefLabel "Item I286"@en-AU ;
    dcat:accessURL <https://www.legislation.gov.au/F2021L00319/2024-04-30/2024-04-30/text/original/epub/OEBPS/document_1/document_1.html#_Toc166158119> ;
    dcat:landingPage "https://www.legislation.gov.au/F2021L00319/2024-04-30/2024-04-30/text/original/epub/OEBPS/document_1/document_1.html#_Toc166158119"^^xsd:anyURI ;
    dcat:theme legcons:Item .

F2021L00319:288 a legcons:Item,
        owl:Class,
        dcat:Resource ;
    rdfs:label "Item - I288 9 16  Application to renew accreditation"@en-AU ;
    dct:isPartOf F2021L00319:287 ;
    dct:isReferencedBy F2021L00319: ;
    rdfs:comment "9 16  Application to renew accreditation - Abrievated Graph Key: I288"@en-AU ;
    skos:definition "9 16  Application to renew accreditation"@en-AU ;
    skos:narrower F2021L00319:287 ;
    skos:prefLabel "Item I288"@en-AU ;
    dcat:accessURL <https://www.legislation.gov.au/F2021L00319/2024-04-30/2024-04-30/text/original/epub/OEBPS/document_1/document_1.html#_Toc166158121> ;
    dcat:landingPage "https://www.legislation.gov.au/F2021L00319/2024-04-30/2024-04-30/text/original/epub/OEBPS/document_1/document_1.html#_Toc166158121"^^xsd:anyURI ;
    dcat:theme legcons:Item .

F2021L00319:289 a legcons:Item,
        owl:Class,
        dcat:Resource ;
    rdfs:label "Item - I289 9 17  Secretary must decide whether to renew accreditation"@en-AU ;
    dct:isPartOf F2021L00319:287 ;
    dct:isReferencedBy F2021L00319: ;
    rdfs:comment "9 17  Secretary must decide whether to renew accreditation - Abrievated Graph Key: I289"@en-AU ;
    skos:definition "9 17  Secretary must decide whether to renew accreditation"@en-AU ;
    skos:narrower F2021L00319:287 ;
    skos:prefLabel "Item I289"@en-AU ;
    dcat:accessURL <https://www.legislation.gov.au/F2021L00319/2024-04-30/2024-04-30/text/original/epub/OEBPS/document_1/document_1.html#_Toc166158122> ;
    dcat:landingPage "https://www.legislation.gov.au/F2021L00319/2024-04-30/2024-04-30/text/original/epub/OEBPS/document_1/document_1.html#_Toc166158122"^^xsd:anyURI ;
    dcat:theme legcons:Item .

F2021L00319:29 a legcons:Item,
        owl:Class,
        dcat:Resource ;
    rdfs:label "Item - I29 2 14  When government certificate may be issued in relation to prescribed livestock prescribed live animals or prescribed animal reproductive material"@en-AU ;
    dct:isPartOf F2021L00319:27 ;
    dct:isReferencedBy F2021L00319: ;
    rdfs:comment "2 14  When government certificate may be issued in relation to prescribed livestock prescribed live animals or prescribed animal reproductive material - Abrievated Graph Key: I29"@en-AU ;
    skos:definition "2 14  When government certificate may be issued in relation to prescribed livestock prescribed live animals or prescribed animal reproductive material"@en-AU ;
    skos:narrower F2021L00319:27 ;
    skos:prefLabel "Item I29"@en-AU ;
    dcat:accessURL <https://www.legislation.gov.au/F2021L00319/2024-04-30/2024-04-30/text/original/epub/OEBPS/document_1/document_1.html#_Toc166157862> ;
    dcat:landingPage "https://www.legislation.gov.au/F2021L00319/2024-04-30/2024-04-30/text/original/epub/OEBPS/document_1/document_1.html#_Toc166157862"^^xsd:anyURI ;
    dcat:theme legcons:Item .

F2021L00319:291 a legcons:Item,
        owl:Class,
        dcat:Resource ;
    rdfs:label "Item - I291 9 18  Application by accredited veterinarian"@en-AU ;
    dct:isPartOf F2021L00319:290 ;
    dct:isReferencedBy F2021L00319: ;
    rdfs:comment "9 18  Application by accredited veterinarian - Abrievated Graph Key: I291"@en-AU ;
    skos:definition "9 18  Application by accredited veterinarian"@en-AU ;
    skos:narrower F2021L00319:290 ;
    skos:prefLabel "Item I291"@en-AU ;
    dcat:accessURL <https://www.legislation.gov.au/F2021L00319/2024-04-30/2024-04-30/text/original/epub/OEBPS/document_1/document_1.html#_Toc166158124> ;
    dcat:landingPage "https://www.legislation.gov.au/F2021L00319/2024-04-30/2024-04-30/text/original/epub/OEBPS/document_1/document_1.html#_Toc166158124"^^xsd:anyURI ;
    dcat:theme legcons:Item .

F2021L00319:292 a legcons:Item,
        owl:Class,
        dcat:Resource ;
    rdfs:label "Item - I292 9 19  Secretary may make variations in relation to accreditation"@en-AU ;
    dct:isPartOf F2021L00319:290 ;
    dct:isReferencedBy F2021L00319: ;
    rdfs:comment "9 19  Secretary may make variations in relation to accreditation - Abrievated Graph Key: I292"@en-AU ;
    skos:definition "9 19  Secretary may make variations in relation to accreditation"@en-AU ;
    skos:narrower F2021L00319:290 ;
    skos:prefLabel "Item I292"@en-AU ;
    dcat:accessURL <https://www.legislation.gov.au/F2021L00319/2024-04-30/2024-04-30/text/original/epub/OEBPS/document_1/document_1.html#_Toc166158125> ;
    dcat:landingPage "https://www.legislation.gov.au/F2021L00319/2024-04-30/2024-04-30/text/original/epub/OEBPS/document_1/document_1.html#_Toc166158125"^^xsd:anyURI ;
    dcat:theme legcons:Item .

F2021L00319:294 a legcons:Item,
        owl:Class,
        dcat:Resource ;
    rdfs:label "Item - I294 9 20  Secretary may suspend accreditation of veterinarian in whole or in part"@en-AU ;
    dct:isPartOf F2021L00319:293 ;
    dct:isReferencedBy F2021L00319: ;
    rdfs:comment "9 20  Secretary may suspend accreditation of veterinarian in whole or in part - Abrievated Graph Key: I294"@en-AU ;
    skos:definition "9 20  Secretary may suspend accreditation of veterinarian in whole or in part"@en-AU ;
    skos:narrower F2021L00319:293 ;
    skos:prefLabel "Item I294"@en-AU ;
    dcat:accessURL <https://www.legislation.gov.au/F2021L00319/2024-04-30/2024-04-30/text/original/epub/OEBPS/document_1/document_1.html#_Toc166158127> ;
    dcat:landingPage "https://www.legislation.gov.au/F2021L00319/2024-04-30/2024-04-30/text/original/epub/OEBPS/document_1/document_1.html#_Toc166158127"^^xsd:anyURI ;
    dcat:theme legcons:Item .

F2021L00319:295 a legcons:Item,
        owl:Class,
        dcat:Resource ;
    rdfs:label "Item - I295 9 21  Notice and start of suspension"@en-AU ;
    dct:isPartOf F2021L00319:293 ;
    dct:isReferencedBy F2021L00319: ;
    rdfs:comment "9 21  Notice and start of suspension - Abrievated Graph Key: I295"@en-AU ;
    skos:definition "9 21  Notice and start of suspension"@en-AU ;
    skos:narrower F2021L00319:293 ;
    skos:prefLabel "Item I295"@en-AU ;
    dcat:accessURL <https://www.legislation.gov.au/F2021L00319/2024-04-30/2024-04-30/text/original/epub/OEBPS/document_1/document_1.html#_Toc166158128> ;
    dcat:landingPage "https://www.legislation.gov.au/F2021L00319/2024-04-30/2024-04-30/text/original/epub/OEBPS/document_1/document_1.html#_Toc166158128"^^xsd:anyURI ;
    dcat:theme legcons:Item .

F2021L00319:296 a legcons:Item,
        owl:Class,
        dcat:Resource ;
    rdfs:label "Item - I296 9 22  Revocation of suspension"@en-AU ;
    dct:isPartOf F2021L00319:293 ;
    dct:isReferencedBy F2021L00319: ;
    rdfs:comment "9 22  Revocation of suspension - Abrievated Graph Key: I296"@en-AU ;
    skos:definition "9 22  Revocation of suspension"@en-AU ;
    skos:narrower F2021L00319:293 ;
    skos:prefLabel "Item I296"@en-AU ;
    dcat:accessURL <https://www.legislation.gov.au/F2021L00319/2024-04-30/2024-04-30/text/original/epub/OEBPS/document_1/document_1.html#_Toc166158129> ;
    dcat:landingPage "https://www.legislation.gov.au/F2021L00319/2024-04-30/2024-04-30/text/original/epub/OEBPS/document_1/document_1.html#_Toc166158129"^^xsd:anyURI ;
    dcat:theme legcons:Item .

F2021L00319:297 a legcons:Item,
        owl:Class,
        dcat:Resource ;
    rdfs:label "Item - I297 9 23  Effect of suspension"@en-AU ;
    dct:isPartOf F2021L00319:293 ;
    dct:isReferencedBy F2021L00319: ;
    rdfs:comment "9 23  Effect of suspension - Abrievated Graph Key: I297"@en-AU ;
    skos:definition "9 23  Effect of suspension"@en-AU ;
    skos:narrower F2021L00319:293 ;
    skos:prefLabel "Item I297"@en-AU ;
    dcat:accessURL <https://www.legislation.gov.au/F2021L00319/2024-04-30/2024-04-30/text/original/epub/OEBPS/document_1/document_1.html#_Toc166158130> ;
    dcat:landingPage "https://www.legislation.gov.au/F2021L00319/2024-04-30/2024-04-30/text/original/epub/OEBPS/document_1/document_1.html#_Toc166158130"^^xsd:anyURI ;
    dcat:theme legcons:Item .

F2021L00319:299 a legcons:Item,
        owl:Class,
        dcat:Resource ;
    rdfs:label "Item - I299 9 24  Secretary may revoke accreditation of veterinarian"@en-AU ;
    dct:isPartOf F2021L00319:298 ;
    dct:isReferencedBy F2021L00319: ;
    rdfs:comment "9 24  Secretary may revoke accreditation of veterinarian - Abrievated Graph Key: I299"@en-AU ;
    skos:definition "9 24  Secretary may revoke accreditation of veterinarian"@en-AU ;
    skos:narrower F2021L00319:298 ;
    skos:prefLabel "Item I299"@en-AU ;
    dcat:accessURL <https://www.legislation.gov.au/F2021L00319/2024-04-30/2024-04-30/text/original/epub/OEBPS/document_1/document_1.html#_Toc166158132> ;
    dcat:landingPage "https://www.legislation.gov.au/F2021L00319/2024-04-30/2024-04-30/text/original/epub/OEBPS/document_1/document_1.html#_Toc166158132"^^xsd:anyURI ;
    dcat:theme legcons:Item .

F2021L00319:3 a legcons:Item,
        owl:Class,
        dcat:Resource ;
    rdfs:label "Item - I3 1 1  Name"@en-AU ;
    dct:isPartOf F2021L00319:1 ;
    dct:isReferencedBy F2021L00319: ;
    rdfs:comment "1 1  Name - Abrievated Graph Key: I3"@en-AU ;
    skos:definition "1 1  Name"@en-AU ;
    skos:narrower F2021L00319:1 ;
    skos:prefLabel "Item I3"@en-AU ;
    dcat:accessURL <https://www.legislation.gov.au/F2021L00319/2024-04-30/2024-04-30/text/original/epub/OEBPS/document_1/document_1.html#_Toc166157836> ;
    dcat:landingPage "https://www.legislation.gov.au/F2021L00319/2024-04-30/2024-04-30/text/original/epub/OEBPS/document_1/document_1.html#_Toc166157836"^^xsd:anyURI ;
    dcat:theme legcons:Item .

F2021L00319:30 a legcons:Item,
        owl:Class,
        dcat:Resource ;
    rdfs:label "Item - I30 2 14 A  Application for new government certificate if original government certificate is revoked"@en-AU ;
    dct:isPartOf F2021L00319:27 ;
    dct:isReferencedBy F2021L00319: ;
    rdfs:comment "2 14 A  Application for new government certificate if original government certificate is revoked - Abrievated Graph Key: I30"@en-AU ;
    skos:definition "2 14 A  Application for new government certificate if original government certificate is revoked"@en-AU ;
    skos:narrower F2021L00319:27 ;
    skos:prefLabel "Item I30"@en-AU ;
    dcat:accessURL <https://www.legislation.gov.au/F2021L00319/2024-04-30/2024-04-30/text/original/epub/OEBPS/document_1/document_1.html#_Toc166157863> ;
    dcat:landingPage "https://www.legislation.gov.au/F2021L00319/2024-04-30/2024-04-30/text/original/epub/OEBPS/document_1/document_1.html#_Toc166157863"^^xsd:anyURI ;
    dcat:theme legcons:Item .

F2021L00319:300 a legcons:Item,
        owl:Class,
        dcat:Resource ;
    rdfs:label "Item - I300 9 25  Notice of revocation"@en-AU ;
    dct:isPartOf F2021L00319:298 ;
    dct:isReferencedBy F2021L00319: ;
    rdfs:comment "9 25  Notice of revocation - Abrievated Graph Key: I300"@en-AU ;
    skos:definition "9 25  Notice of revocation"@en-AU ;
    skos:narrower F2021L00319:298 ;
    skos:prefLabel "Item I300"@en-AU ;
    dcat:accessURL <https://www.legislation.gov.au/F2021L00319/2024-04-30/2024-04-30/text/original/epub/OEBPS/document_1/document_1.html#_Toc166158133> ;
    dcat:landingPage "https://www.legislation.gov.au/F2021L00319/2024-04-30/2024-04-30/text/original/epub/OEBPS/document_1/document_1.html#_Toc166158133"^^xsd:anyURI ;
    dcat:theme legcons:Item .

F2021L00319:302 a legcons:Item,
        owl:Class,
        dcat:Resource ;
    rdfs:label "Item - I302 9 26  Records"@en-AU ;
    dct:isPartOf F2021L00319:301 ;
    dct:isReferencedBy F2021L00319: ;
    rdfs:comment "9 26  Records - Abrievated Graph Key: I302"@en-AU ;
    skos:definition "9 26  Records"@en-AU ;
    skos:narrower F2021L00319:301 ;
    skos:prefLabel "Item I302"@en-AU ;
    dcat:accessURL <https://www.legislation.gov.au/F2021L00319/2024-04-30/2024-04-30/text/original/epub/OEBPS/document_1/document_1.html#_Toc166158135> ;
    dcat:landingPage "https://www.legislation.gov.au/F2021L00319/2024-04-30/2024-04-30/text/original/epub/OEBPS/document_1/document_1.html#_Toc166158135"^^xsd:anyURI ;
    dcat:theme legcons:Item .

F2021L00319:303 a legcons:Item,
        owl:Class,
        dcat:Resource ;
    rdfs:label "Item - I303 9 27  Reports"@en-AU ;
    dct:isPartOf F2021L00319:301 ;
    dct:isReferencedBy F2021L00319: ;
    rdfs:comment "9 27  Reports - Abrievated Graph Key: I303"@en-AU ;
    skos:definition "9 27  Reports"@en-AU ;
    skos:narrower F2021L00319:301 ;
    skos:prefLabel "Item I303"@en-AU ;
    dcat:accessURL <https://www.legislation.gov.au/F2021L00319/2024-04-30/2024-04-30/text/original/epub/OEBPS/document_1/document_1.html#_Toc166158136> ;
    dcat:landingPage "https://www.legislation.gov.au/F2021L00319/2024-04-30/2024-04-30/text/original/epub/OEBPS/document_1/document_1.html#_Toc166158136"^^xsd:anyURI ;
    dcat:theme legcons:Item .

F2021L00319:305 a legcons:Item,
        owl:Class,
        dcat:Resource ;
    rdfs:label "Item - I305 9 28  Fit and proper person test"@en-AU ;
    dct:isPartOf F2021L00319:304 ;
    dct:isReferencedBy F2021L00319: ;
    rdfs:comment "9 28  Fit and proper person test - Abrievated Graph Key: I305"@en-AU ;
    skos:definition "9 28  Fit and proper person test"@en-AU ;
    skos:narrower F2021L00319:304 ;
    skos:prefLabel "Item I305"@en-AU ;
    dcat:accessURL <https://www.legislation.gov.au/F2021L00319/2024-04-30/2024-04-30/text/original/epub/OEBPS/document_1/document_1.html#_Toc166158138> ;
    dcat:landingPage "https://www.legislation.gov.au/F2021L00319/2024-04-30/2024-04-30/text/original/epub/OEBPS/document_1/document_1.html#_Toc166158138"^^xsd:anyURI ;
    dcat:theme legcons:Item .

F2021L00319:307 a legcons:Item,
        owl:Class,
        dcat:Resource ;
    rdfs:label "Item - I307 9 29  Applications to which this Division applies"@en-AU ;
    dct:isPartOf F2021L00319:306 ;
    dct:isReferencedBy F2021L00319: ;
    rdfs:comment "9 29  Applications to which this Division applies - Abrievated Graph Key: I307"@en-AU ;
    skos:definition "9 29  Applications to which this Division applies"@en-AU ;
    skos:narrower F2021L00319:306 ;
    skos:prefLabel "Item I307"@en-AU ;
    dcat:accessURL <https://www.legislation.gov.au/F2021L00319/2024-04-30/2024-04-30/text/original/epub/OEBPS/document_1/document_1.html#_Toc166158140> ;
    dcat:landingPage "https://www.legislation.gov.au/F2021L00319/2024-04-30/2024-04-30/text/original/epub/OEBPS/document_1/document_1.html#_Toc166158140"^^xsd:anyURI ;
    dcat:theme legcons:Item .

F2021L00319:308 a legcons:Item,
        owl:Class,
        dcat:Resource ;
    rdfs:label "Item - I308 9 30  Requirements for applications"@en-AU ;
    dct:isPartOf F2021L00319:306 ;
    dct:isReferencedBy F2021L00319: ;
    rdfs:comment "9 30  Requirements for applications - Abrievated Graph Key: I308"@en-AU ;
    skos:definition "9 30  Requirements for applications"@en-AU ;
    skos:narrower F2021L00319:306 ;
    skos:prefLabel "Item I308"@en-AU ;
    dcat:accessURL <https://www.legislation.gov.au/F2021L00319/2024-04-30/2024-04-30/text/original/epub/OEBPS/document_1/document_1.html#_Toc166158141> ;
    dcat:landingPage "https://www.legislation.gov.au/F2021L00319/2024-04-30/2024-04-30/text/original/epub/OEBPS/document_1/document_1.html#_Toc166158141"^^xsd:anyURI ;
    dcat:theme legcons:Item .

F2021L00319:309 a legcons:Item,
        owl:Class,
        dcat:Resource ;
    rdfs:label "Item - I309 9 31  Dealing with applications"@en-AU ;
    dct:isPartOf F2021L00319:306 ;
    dct:isReferencedBy F2021L00319: ;
    rdfs:comment "9 31  Dealing with applications - Abrievated Graph Key: I309"@en-AU ;
    skos:definition "9 31  Dealing with applications"@en-AU ;
    skos:narrower F2021L00319:306 ;
    skos:prefLabel "Item I309"@en-AU ;
    dcat:accessURL <https://www.legislation.gov.au/F2021L00319/2024-04-30/2024-04-30/text/original/epub/OEBPS/document_1/document_1.html#_Toc166158142> ;
    dcat:landingPage "https://www.legislation.gov.au/F2021L00319/2024-04-30/2024-04-30/text/original/epub/OEBPS/document_1/document_1.html#_Toc166158142"^^xsd:anyURI ;
    dcat:theme legcons:Item .

F2021L00319:31 a legcons:Item,
        owl:Class,
        dcat:Resource ;
    rdfs:label "Item - I31 2 15  Circumstances for refusing to issue government certificate"@en-AU ;
    dct:isPartOf F2021L00319:27 ;
    dct:isReferencedBy F2021L00319: ;
    rdfs:comment "2 15  Circumstances for refusing to issue government certificate - Abrievated Graph Key: I31"@en-AU ;
    skos:definition "2 15  Circumstances for refusing to issue government certificate"@en-AU ;
    skos:narrower F2021L00319:27 ;
    skos:prefLabel "Item I31"@en-AU ;
    dcat:accessURL <https://www.legislation.gov.au/F2021L00319/2024-04-30/2024-04-30/text/original/epub/OEBPS/document_1/document_1.html#_Toc166157864> ;
    dcat:landingPage "https://www.legislation.gov.au/F2021L00319/2024-04-30/2024-04-30/text/original/epub/OEBPS/document_1/document_1.html#_Toc166157864"^^xsd:anyURI ;
    dcat:theme legcons:Item .

F2021L00319:312 a legcons:Item,
        owl:Class,
        dcat:Resource ;
    rdfs:label "Item - I312 9 32  Purpose of this Part"@en-AU ;
    dct:isPartOf F2021L00319:311 ;
    dct:isReferencedBy F2021L00319: ;
    rdfs:comment "9 32  Purpose of this Part - Abrievated Graph Key: I312"@en-AU ;
    skos:definition "9 32  Purpose of this Part"@en-AU ;
    skos:narrower F2021L00319:311 ;
    skos:prefLabel "Item I312"@en-AU ;
    dcat:accessURL <https://www.legislation.gov.au/F2021L00319/2024-04-30/2024-04-30/text/original/epub/OEBPS/document_1/document_1.html#_Toc166158145> ;
    dcat:landingPage "https://www.legislation.gov.au/F2021L00319/2024-04-30/2024-04-30/text/original/epub/OEBPS/document_1/document_1.html#_Toc166158145"^^xsd:anyURI ;
    dcat:theme legcons:Item .

F2021L00319:315 a legcons:Item,
        owl:Class,
        dcat:Resource ;
    rdfs:label "Item - I315 9 33  Application by exporter for approval of program of export operations"@en-AU ;
    dct:isPartOf F2021L00319:314 ;
    dct:isReferencedBy F2021L00319: ;
    rdfs:comment "9 33  Application by exporter for approval of program of export operations - Abrievated Graph Key: I315"@en-AU ;
    skos:definition "9 33  Application by exporter for approval of program of export operations"@en-AU ;
    skos:narrower F2021L00319:314 ;
    skos:prefLabel "Item I315"@en-AU ;
    dcat:accessURL <https://www.legislation.gov.au/F2021L00319/2024-04-30/2024-04-30/text/original/epub/OEBPS/document_1/document_1.html#_Toc166158148> ;
    dcat:landingPage "https://www.legislation.gov.au/F2021L00319/2024-04-30/2024-04-30/text/original/epub/OEBPS/document_1/document_1.html#_Toc166158148"^^xsd:anyURI ;
    dcat:theme legcons:Item .

F2021L00319:316 a legcons:Item,
        owl:Class,
        dcat:Resource ;
    rdfs:label "Item - I316 9 34  Assessment of application and Secretarys decision"@en-AU ;
    dct:isPartOf F2021L00319:314 ;
    dct:isReferencedBy F2021L00319: ;
    rdfs:comment "9 34  Assessment of application and Secretarys decision - Abrievated Graph Key: I316"@en-AU ;
    skos:definition "9 34  Assessment of application and Secretarys decision"@en-AU ;
    skos:narrower F2021L00319:314 ;
    skos:prefLabel "Item I316"@en-AU ;
    dcat:accessURL <https://www.legislation.gov.au/F2021L00319/2024-04-30/2024-04-30/text/original/epub/OEBPS/document_1/document_1.html#_Toc166158149> ;
    dcat:landingPage "https://www.legislation.gov.au/F2021L00319/2024-04-30/2024-04-30/text/original/epub/OEBPS/document_1/document_1.html#_Toc166158149"^^xsd:anyURI ;
    dcat:theme legcons:Item .

F2021L00319:317 a legcons:Item,
        owl:Class,
        dcat:Resource ;
    rdfs:label "Item - I317 9 35  Period of effect of approved export program"@en-AU ;
    dct:isPartOf F2021L00319:314 ;
    dct:isReferencedBy F2021L00319: ;
    rdfs:comment "9 35  Period of effect of approved export program - Abrievated Graph Key: I317"@en-AU ;
    skos:definition "9 35  Period of effect of approved export program"@en-AU ;
    skos:narrower F2021L00319:314 ;
    skos:prefLabel "Item I317"@en-AU ;
    dcat:accessURL <https://www.legislation.gov.au/F2021L00319/2024-04-30/2024-04-30/text/original/epub/OEBPS/document_1/document_1.html#_Toc166158150> ;
    dcat:landingPage "https://www.legislation.gov.au/F2021L00319/2024-04-30/2024-04-30/text/original/epub/OEBPS/document_1/document_1.html#_Toc166158150"^^xsd:anyURI ;
    dcat:theme legcons:Item .

F2021L00319:319 a legcons:Item,
        owl:Class,
        dcat:Resource ;
    rdfs:label "Item - I319 9 36  Holder may apply for approval of variation of approved export program"@en-AU ;
    dct:isPartOf F2021L00319:318 ;
    dct:isReferencedBy F2021L00319: ;
    rdfs:comment "9 36  Holder may apply for approval of variation of approved export program - Abrievated Graph Key: I319"@en-AU ;
    skos:definition "9 36  Holder may apply for approval of variation of approved export program"@en-AU ;
    skos:narrower F2021L00319:318 ;
    skos:prefLabel "Item I319"@en-AU ;
    dcat:accessURL <https://www.legislation.gov.au/F2021L00319/2024-04-30/2024-04-30/text/original/epub/OEBPS/document_1/document_1.html#_Toc166158152> ;
    dcat:landingPage "https://www.legislation.gov.au/F2021L00319/2024-04-30/2024-04-30/text/original/epub/OEBPS/document_1/document_1.html#_Toc166158152"^^xsd:anyURI ;
    dcat:theme legcons:Item .

F2021L00319:32 a legcons:Item,
        owl:Class,
        dcat:Resource ;
    rdfs:label "Item - I32 2 16  Changes that require holder of certificate to give additional or corrected information to issuing body"@en-AU ;
    dct:isPartOf F2021L00319:27 ;
    dct:isReferencedBy F2021L00319: ;
    rdfs:comment "2 16  Changes that require holder of certificate to give additional or corrected information to issuing body - Abrievated Graph Key: I32"@en-AU ;
    skos:definition "2 16  Changes that require holder of certificate to give additional or corrected information to issuing body"@en-AU ;
    skos:narrower F2021L00319:27 ;
    skos:prefLabel "Item I32"@en-AU ;
    dcat:accessURL <https://www.legislation.gov.au/F2021L00319/2024-04-30/2024-04-30/text/original/epub/OEBPS/document_1/document_1.html#_Toc166157865> ;
    dcat:landingPage "https://www.legislation.gov.au/F2021L00319/2024-04-30/2024-04-30/text/original/epub/OEBPS/document_1/document_1.html#_Toc166157865"^^xsd:anyURI ;
    dcat:theme legcons:Item .

F2021L00319:320 a legcons:Item,
        owl:Class,
        dcat:Resource ;
    rdfs:label "Item - I320 9 37  Secretary may require holder to vary approved export program"@en-AU ;
    dct:isPartOf F2021L00319:318 ;
    dct:isReferencedBy F2021L00319: ;
    rdfs:comment "9 37  Secretary may require holder to vary approved export program - Abrievated Graph Key: I320"@en-AU ;
    skos:definition "9 37  Secretary may require holder to vary approved export program"@en-AU ;
    skos:narrower F2021L00319:318 ;
    skos:prefLabel "Item I320"@en-AU ;
    dcat:accessURL <https://www.legislation.gov.au/F2021L00319/2024-04-30/2024-04-30/text/original/epub/OEBPS/document_1/document_1.html#_Toc166158153> ;
    dcat:landingPage "https://www.legislation.gov.au/F2021L00319/2024-04-30/2024-04-30/text/original/epub/OEBPS/document_1/document_1.html#_Toc166158153"^^xsd:anyURI ;
    dcat:theme legcons:Item .

F2021L00319:321 a legcons:Item,
        owl:Class,
        dcat:Resource ;
    rdfs:label "Item - I321 9 38  When approved export program includes a variation"@en-AU ;
    dct:isPartOf F2021L00319:318 ;
    dct:isReferencedBy F2021L00319: ;
    rdfs:comment "9 38  When approved export program includes a variation - Abrievated Graph Key: I321"@en-AU ;
    skos:definition "9 38  When approved export program includes a variation"@en-AU ;
    skos:narrower F2021L00319:318 ;
    skos:prefLabel "Item I321"@en-AU ;
    dcat:accessURL <https://www.legislation.gov.au/F2021L00319/2024-04-30/2024-04-30/text/original/epub/OEBPS/document_1/document_1.html#_Toc166158154> ;
    dcat:landingPage "https://www.legislation.gov.au/F2021L00319/2024-04-30/2024-04-30/text/original/epub/OEBPS/document_1/document_1.html#_Toc166158154"^^xsd:anyURI ;
    dcat:theme legcons:Item .

F2021L00319:323 a legcons:Item,
        owl:Class,
        dcat:Resource ;
    rdfs:label "Item - I323 9 39  Holder may request suspension of approved export program"@en-AU ;
    dct:isPartOf F2021L00319:322 ;
    dct:isReferencedBy F2021L00319: ;
    rdfs:comment "9 39  Holder may request suspension of approved export program - Abrievated Graph Key: I323"@en-AU ;
    skos:definition "9 39  Holder may request suspension of approved export program"@en-AU ;
    skos:narrower F2021L00319:322 ;
    skos:prefLabel "Item I323"@en-AU ;
    dcat:accessURL <https://www.legislation.gov.au/F2021L00319/2024-04-30/2024-04-30/text/original/epub/OEBPS/document_1/document_1.html#_Toc166158156> ;
    dcat:landingPage "https://www.legislation.gov.au/F2021L00319/2024-04-30/2024-04-30/text/original/epub/OEBPS/document_1/document_1.html#_Toc166158156"^^xsd:anyURI ;
    dcat:theme legcons:Item .

F2021L00319:324 a legcons:Item,
        owl:Class,
        dcat:Resource ;
    rdfs:label "Item - I324 9 40  Request to revoke suspension"@en-AU ;
    dct:isPartOf F2021L00319:322 ;
    dct:isReferencedBy F2021L00319: ;
    rdfs:comment "9 40  Request to revoke suspension - Abrievated Graph Key: I324"@en-AU ;
    skos:definition "9 40  Request to revoke suspension"@en-AU ;
    skos:narrower F2021L00319:322 ;
    skos:prefLabel "Item I324"@en-AU ;
    dcat:accessURL <https://www.legislation.gov.au/F2021L00319/2024-04-30/2024-04-30/text/original/epub/OEBPS/document_1/document_1.html#_Toc166158157> ;
    dcat:landingPage "https://www.legislation.gov.au/F2021L00319/2024-04-30/2024-04-30/text/original/epub/OEBPS/document_1/document_1.html#_Toc166158157"^^xsd:anyURI ;
    dcat:theme legcons:Item .

F2021L00319:325 a legcons:Item,
        owl:Class,
        dcat:Resource ;
    rdfs:label "Item - I325 9 41  Secretary may suspend approved export program"@en-AU ;
    dct:isPartOf F2021L00319:322 ;
    dct:isReferencedBy F2021L00319: ;
    rdfs:comment "9 41  Secretary may suspend approved export program - Abrievated Graph Key: I325"@en-AU ;
    skos:definition "9 41  Secretary may suspend approved export program"@en-AU ;
    skos:narrower F2021L00319:322 ;
    skos:prefLabel "Item I325"@en-AU ;
    dcat:accessURL <https://www.legislation.gov.au/F2021L00319/2024-04-30/2024-04-30/text/original/epub/OEBPS/document_1/document_1.html#_Toc166158158> ;
    dcat:landingPage "https://www.legislation.gov.au/F2021L00319/2024-04-30/2024-04-30/text/original/epub/OEBPS/document_1/document_1.html#_Toc166158158"^^xsd:anyURI ;
    dcat:theme legcons:Item .

F2021L00319:327 a legcons:Item,
        owl:Class,
        dcat:Resource ;
    rdfs:label "Item - I327 9 42  Holder may request revocation of approved export program"@en-AU ;
    dct:isPartOf F2021L00319:326 ;
    dct:isReferencedBy F2021L00319: ;
    rdfs:comment "9 42  Holder may request revocation of approved export program - Abrievated Graph Key: I327"@en-AU ;
    skos:definition "9 42  Holder may request revocation of approved export program"@en-AU ;
    skos:narrower F2021L00319:326 ;
    skos:prefLabel "Item I327"@en-AU ;
    dcat:accessURL <https://www.legislation.gov.au/F2021L00319/2024-04-30/2024-04-30/text/original/epub/OEBPS/document_1/document_1.html#_Toc166158160> ;
    dcat:landingPage "https://www.legislation.gov.au/F2021L00319/2024-04-30/2024-04-30/text/original/epub/OEBPS/document_1/document_1.html#_Toc166158160"^^xsd:anyURI ;
    dcat:theme legcons:Item .

F2021L00319:328 a legcons:Item,
        owl:Class,
        dcat:Resource ;
    rdfs:label "Item - I328 9 43  Secretary may revoke approved export program"@en-AU ;
    dct:isPartOf F2021L00319:326 ;
    dct:isReferencedBy F2021L00319: ;
    rdfs:comment "9 43  Secretary may revoke approved export program - Abrievated Graph Key: I328"@en-AU ;
    skos:definition "9 43  Secretary may revoke approved export program"@en-AU ;
    skos:narrower F2021L00319:326 ;
    skos:prefLabel "Item I328"@en-AU ;
    dcat:accessURL <https://www.legislation.gov.au/F2021L00319/2024-04-30/2024-04-30/text/original/epub/OEBPS/document_1/document_1.html#_Toc166158161> ;
    dcat:landingPage "https://www.legislation.gov.au/F2021L00319/2024-04-30/2024-04-30/text/original/epub/OEBPS/document_1/document_1.html#_Toc166158161"^^xsd:anyURI ;
    dcat:theme legcons:Item .

F2021L00319:33 a legcons:Item,
        owl:Class,
        dcat:Resource ;
    rdfs:label "Item - I33 2 16 A  Circumstances for revocation of government certificate"@en-AU ;
    dct:isPartOf F2021L00319:27 ;
    dct:isReferencedBy F2021L00319: ;
    rdfs:comment "2 16 A  Circumstances for revocation of government certificate - Abrievated Graph Key: I33"@en-AU ;
    skos:definition "2 16 A  Circumstances for revocation of government certificate"@en-AU ;
    skos:narrower F2021L00319:27 ;
    skos:prefLabel "Item I33"@en-AU ;
    dcat:accessURL <https://www.legislation.gov.au/F2021L00319/2024-04-30/2024-04-30/text/original/epub/OEBPS/document_1/document_1.html#_Toc166157866> ;
    dcat:landingPage "https://www.legislation.gov.au/F2021L00319/2024-04-30/2024-04-30/text/original/epub/OEBPS/document_1/document_1.html#_Toc166157866"^^xsd:anyURI ;
    dcat:theme legcons:Item .

F2021L00319:330 a legcons:Item,
        owl:Class,
        dcat:Resource ;
    rdfs:label "Item - I330 9 43 A  Holder must provide copies of approved export program"@en-AU ;
    dct:isPartOf F2021L00319:329 ;
    dct:isReferencedBy F2021L00319: ;
    rdfs:comment "9 43 A  Holder must provide copies of approved export program - Abrievated Graph Key: I330"@en-AU ;
    skos:definition "9 43 A  Holder must provide copies of approved export program"@en-AU ;
    skos:narrower F2021L00319:329 ;
    skos:prefLabel "Item I330"@en-AU ;
    dcat:accessURL <https://www.legislation.gov.au/F2021L00319/2024-04-30/2024-04-30/text/original/epub/OEBPS/document_1/document_1.html#_Toc166158163> ;
    dcat:landingPage "https://www.legislation.gov.au/F2021L00319/2024-04-30/2024-04-30/text/original/epub/OEBPS/document_1/document_1.html#_Toc166158163"^^xsd:anyURI ;
    dcat:theme legcons:Item .

F2021L00319:332 a legcons:Item,
        owl:Class,
        dcat:Resource ;
    rdfs:label "Item - I332 9 44  Approvals of programs of export operations to be undertaken by authorised officers"@en-AU ;
    dct:isPartOf F2021L00319:331 ;
    dct:isReferencedBy F2021L00319: ;
    rdfs:comment "9 44  Approvals of programs of export operations to be undertaken by authorised officers - Abrievated Graph Key: I332"@en-AU ;
    skos:definition "9 44  Approvals of programs of export operations to be undertaken by authorised officers"@en-AU ;
    skos:narrower F2021L00319:331 ;
    skos:prefLabel "Item I332"@en-AU ;
    dcat:accessURL <https://www.legislation.gov.au/F2021L00319/2024-04-30/2024-04-30/text/original/epub/OEBPS/document_1/document_1.html#_Toc166158165> ;
    dcat:landingPage "https://www.legislation.gov.au/F2021L00319/2024-04-30/2024-04-30/text/original/epub/OEBPS/document_1/document_1.html#_Toc166158165"^^xsd:anyURI ;
    dcat:theme legcons:Item .

F2021L00319:333 a legcons:Item,
        owl:Class,
        dcat:Resource ;
    rdfs:label "Item - I333 9 45  Period of effect of approved export program"@en-AU ;
    dct:isPartOf F2021L00319:331 ;
    dct:isReferencedBy F2021L00319: ;
    rdfs:comment "9 45  Period of effect of approved export program - Abrievated Graph Key: I333"@en-AU ;
    skos:definition "9 45  Period of effect of approved export program"@en-AU ;
    skos:narrower F2021L00319:331 ;
    skos:prefLabel "Item I333"@en-AU ;
    dcat:accessURL <https://www.legislation.gov.au/F2021L00319/2024-04-30/2024-04-30/text/original/epub/OEBPS/document_1/document_1.html#_Toc166158166> ;
    dcat:landingPage "https://www.legislation.gov.au/F2021L00319/2024-04-30/2024-04-30/text/original/epub/OEBPS/document_1/document_1.html#_Toc166158166"^^xsd:anyURI ;
    dcat:theme legcons:Item .

F2021L00319:334 a legcons:Item,
        owl:Class,
        dcat:Resource ;
    rdfs:label "Item - I334 9 46  Secretary may vary approved export program"@en-AU ;
    dct:isPartOf F2021L00319:331 ;
    dct:isReferencedBy F2021L00319: ;
    rdfs:comment "9 46  Secretary may vary approved export program - Abrievated Graph Key: I334"@en-AU ;
    skos:definition "9 46  Secretary may vary approved export program"@en-AU ;
    skos:narrower F2021L00319:331 ;
    skos:prefLabel "Item I334"@en-AU ;
    dcat:accessURL <https://www.legislation.gov.au/F2021L00319/2024-04-30/2024-04-30/text/original/epub/OEBPS/document_1/document_1.html#_Toc166158167> ;
    dcat:landingPage "https://www.legislation.gov.au/F2021L00319/2024-04-30/2024-04-30/text/original/epub/OEBPS/document_1/document_1.html#_Toc166158167"^^xsd:anyURI ;
    dcat:theme legcons:Item .

F2021L00319:336 a legcons:Item,
        owl:Class,
        dcat:Resource ;
    rdfs:label "Item - I336 9 47  Secretary may give direction to exporter in relation to implementation of approved export program"@en-AU ;
    dct:isPartOf F2021L00319:335 ;
    dct:isReferencedBy F2021L00319: ;
    rdfs:comment "9 47  Secretary may give direction to exporter in relation to implementation of approved export program - Abrievated Graph Key: I336"@en-AU ;
    skos:definition "9 47  Secretary may give direction to exporter in relation to implementation of approved export program"@en-AU ;
    skos:narrower F2021L00319:335 ;
    skos:prefLabel "Item I336"@en-AU ;
    dcat:accessURL <https://www.legislation.gov.au/F2021L00319/2024-04-30/2024-04-30/text/original/epub/OEBPS/document_1/document_1.html#_Toc166158169> ;
    dcat:landingPage "https://www.legislation.gov.au/F2021L00319/2024-04-30/2024-04-30/text/original/epub/OEBPS/document_1/document_1.html#_Toc166158169"^^xsd:anyURI ;
    dcat:theme legcons:Item .

F2021L00319:337 a legcons:Item,
        owl:Class,
        dcat:Resource ;
    rdfs:label "Item - I337 9 48  Secretary may publish information in records and reports in relation to approved export programs"@en-AU ;
    dct:isPartOf F2021L00319:335 ;
    dct:isReferencedBy F2021L00319: ;
    rdfs:comment "9 48  Secretary may publish information in records and reports in relation to approved export programs - Abrievated Graph Key: I337"@en-AU ;
    skos:definition "9 48  Secretary may publish information in records and reports in relation to approved export programs"@en-AU ;
    skos:narrower F2021L00319:335 ;
    skos:prefLabel "Item I337"@en-AU ;
    dcat:accessURL <https://www.legislation.gov.au/F2021L00319/2024-04-30/2024-04-30/text/original/epub/OEBPS/document_1/document_1.html#_Toc166158170> ;
    dcat:landingPage "https://www.legislation.gov.au/F2021L00319/2024-04-30/2024-04-30/text/original/epub/OEBPS/document_1/document_1.html#_Toc166158170"^^xsd:anyURI ;
    dcat:theme legcons:Item .

F2021L00319:339 a legcons:Item,
        owl:Class,
        dcat:Resource ;
    rdfs:label "Item - I339 9 49  Circumstances in which exporter must allow accredited veterinarian or authorised officer to accompany livestock"@en-AU ;
    dct:isPartOf F2021L00319:338 ;
    dct:isReferencedBy F2021L00319: ;
    rdfs:comment "9 49  Circumstances in which exporter must allow accredited veterinarian or authorised officer to accompany livestock - Abrievated Graph Key: I339"@en-AU ;
    skos:definition "9 49  Circumstances in which exporter must allow accredited veterinarian or authorised officer to accompany livestock"@en-AU ;
    skos:narrower F2021L00319:338 ;
    skos:prefLabel "Item I339"@en-AU ;
    dcat:accessURL <https://www.legislation.gov.au/F2021L00319/2024-04-30/2024-04-30/text/original/epub/OEBPS/document_1/document_1.html#_Toc166158172> ;
    dcat:landingPage "https://www.legislation.gov.au/F2021L00319/2024-04-30/2024-04-30/text/original/epub/OEBPS/document_1/document_1.html#_Toc166158172"^^xsd:anyURI ;
    dcat:theme legcons:Item .

F2021L00319:34 a legcons:Item,
        owl:Class,
        dcat:Resource ;
    rdfs:label "Item - I34 2 17  Return of government certificate"@en-AU ;
    dct:isPartOf F2021L00319:27 ;
    dct:isReferencedBy F2021L00319: ;
    rdfs:comment "2 17  Return of government certificate - Abrievated Graph Key: I34"@en-AU ;
    skos:definition "2 17  Return of government certificate"@en-AU ;
    skos:narrower F2021L00319:27 ;
    skos:prefLabel "Item I34"@en-AU ;
    dcat:accessURL <https://www.legislation.gov.au/F2021L00319/2024-04-30/2024-04-30/text/original/epub/OEBPS/document_1/document_1.html#_Toc166157867> ;
    dcat:landingPage "https://www.legislation.gov.au/F2021L00319/2024-04-30/2024-04-30/text/original/epub/OEBPS/document_1/document_1.html#_Toc166157867"^^xsd:anyURI ;
    dcat:theme legcons:Item .

F2021L00319:340 a legcons:Item,
        owl:Class,
        dcat:Resource ;
    rdfs:label "Item - I340 9 50  Inconsistency between Secretarys approved export program and exporters approved export program"@en-AU ;
    dct:isPartOf F2021L00319:338 ;
    dct:isReferencedBy F2021L00319: ;
    rdfs:comment "9 50  Inconsistency between Secretarys approved export program and exporters approved export program - Abrievated Graph Key: I340"@en-AU ;
    skos:definition "9 50  Inconsistency between Secretarys approved export program and exporters approved export program"@en-AU ;
    skos:narrower F2021L00319:338 ;
    skos:prefLabel "Item I340"@en-AU ;
    dcat:accessURL <https://www.legislation.gov.au/F2021L00319/2024-04-30/2024-04-30/text/original/epub/OEBPS/document_1/document_1.html#_Toc166158173> ;
    dcat:landingPage "https://www.legislation.gov.au/F2021L00319/2024-04-30/2024-04-30/text/original/epub/OEBPS/document_1/document_1.html#_Toc166158173"^^xsd:anyURI ;
    dcat:theme legcons:Item .

F2021L00319:342 a legcons:Item,
        owl:Class,
        dcat:Resource ;
    rdfs:label "Item - I342 9 51  Powers of Secretary that must not be delegated"@en-AU ;
    dct:isPartOf F2021L00319:341 ;
    dct:isReferencedBy F2021L00319: ;
    rdfs:comment "9 51  Powers of Secretary that must not be delegated - Abrievated Graph Key: I342"@en-AU ;
    skos:definition "9 51  Powers of Secretary that must not be delegated"@en-AU ;
    skos:narrower F2021L00319:341 ;
    skos:prefLabel "Item I342"@en-AU ;
    dcat:accessURL <https://www.legislation.gov.au/F2021L00319/2024-04-30/2024-04-30/text/original/epub/OEBPS/document_1/document_1.html#_Toc166158175> ;
    dcat:landingPage "https://www.legislation.gov.au/F2021L00319/2024-04-30/2024-04-30/text/original/epub/OEBPS/document_1/document_1.html#_Toc166158175"^^xsd:anyURI ;
    dcat:theme legcons:Item .

F2021L00319:343 a legcons:Item,
        owl:Class,
        dcat:Resource ;
    rdfs:label "Item - I343 9 52  Powers of Secretary that must not be subdelegated"@en-AU ;
    dct:isPartOf F2021L00319:341 ;
    dct:isReferencedBy F2021L00319: ;
    rdfs:comment "9 52  Powers of Secretary that must not be subdelegated - Abrievated Graph Key: I343"@en-AU ;
    skos:definition "9 52  Powers of Secretary that must not be subdelegated"@en-AU ;
    skos:narrower F2021L00319:341 ;
    skos:prefLabel "Item I343"@en-AU ;
    dcat:accessURL <https://www.legislation.gov.au/F2021L00319/2024-04-30/2024-04-30/text/original/epub/OEBPS/document_1/document_1.html#_Toc166158176> ;
    dcat:landingPage "https://www.legislation.gov.au/F2021L00319/2024-04-30/2024-04-30/text/original/epub/OEBPS/document_1/document_1.html#_Toc166158176"^^xsd:anyURI ;
    dcat:theme legcons:Item .

F2021L00319:345 a legcons:Item,
        owl:Class,
        dcat:Resource ;
    rdfs:label "Item - I345 9 53  Purpose of this Part"@en-AU ;
    dct:isPartOf F2021L00319:344 ;
    dct:isReferencedBy F2021L00319: ;
    rdfs:comment "9 53  Purpose of this Part - Abrievated Graph Key: I345"@en-AU ;
    skos:definition "9 53  Purpose of this Part"@en-AU ;
    skos:narrower F2021L00319:344 ;
    skos:prefLabel "Item I345"@en-AU ;
    dcat:accessURL <https://www.legislation.gov.au/F2021L00319/2024-04-30/2024-04-30/text/original/epub/OEBPS/document_1/document_1.html#_Toc166158178> ;
    dcat:landingPage "https://www.legislation.gov.au/F2021L00319/2024-04-30/2024-04-30/text/original/epub/OEBPS/document_1/document_1.html#_Toc166158178"^^xsd:anyURI ;
    dcat:theme legcons:Item .

F2021L00319:346 a legcons:Item,
        owl:Class,
        dcat:Resource ;
    rdfs:label "Item - I346 9 54  Power to give orders in relation to prescribed livestock for export"@en-AU ;
    dct:isPartOf F2021L00319:344 ;
    dct:isReferencedBy F2021L00319: ;
    rdfs:comment "9 54  Power to give orders in relation to prescribed livestock for export - Abrievated Graph Key: I346"@en-AU ;
    skos:definition "9 54  Power to give orders in relation to prescribed livestock for export"@en-AU ;
    skos:narrower F2021L00319:344 ;
    skos:prefLabel "Item I346"@en-AU ;
    dcat:accessURL <https://www.legislation.gov.au/F2021L00319/2024-04-30/2024-04-30/text/original/epub/OEBPS/document_1/document_1.html#_Toc166158179> ;
    dcat:landingPage "https://www.legislation.gov.au/F2021L00319/2024-04-30/2024-04-30/text/original/epub/OEBPS/document_1/document_1.html#_Toc166158179"^^xsd:anyURI ;
    dcat:theme legcons:Item .

F2021L00319:348 a legcons:Item,
        owl:Class,
        dcat:Resource ;
    rdfs:label "Item - I348 10 1  Samples taken in exercising monitoring or investigation powers"@en-AU ;
    dct:isPartOf F2021L00319:347 ;
    dct:isReferencedBy F2021L00319: ;
    rdfs:comment "10 1  Samples taken in exercising monitoring or investigation powers - Abrievated Graph Key: I348"@en-AU ;
    skos:definition "10 1  Samples taken in exercising monitoring or investigation powers"@en-AU ;
    skos:narrower F2021L00319:347 ;
    skos:prefLabel "Item I348"@en-AU ;
    dcat:accessURL <https://www.legislation.gov.au/F2021L00319/2024-04-30/2024-04-30/text/original/epub/OEBPS/document_1/document_1.html#_Toc166158181> ;
    dcat:landingPage "https://www.legislation.gov.au/F2021L00319/2024-04-30/2024-04-30/text/original/epub/OEBPS/document_1/document_1.html#_Toc166158181"^^xsd:anyURI ;
    dcat:theme legcons:Item .

F2021L00319:349 a legcons:Item,
        owl:Class,
        dcat:Resource ;
    rdfs:label "Item - I349 10 2  Dealing with things seized in exercising investigation powers"@en-AU ;
    dct:isPartOf F2021L00319:347 ;
    dct:isReferencedBy F2021L00319: ;
    rdfs:comment "10 2  Dealing with things seized in exercising investigation powers - Abrievated Graph Key: I349"@en-AU ;
    skos:definition "10 2  Dealing with things seized in exercising investigation powers"@en-AU ;
    skos:narrower F2021L00319:347 ;
    skos:prefLabel "Item I349"@en-AU ;
    dcat:accessURL <https://www.legislation.gov.au/F2021L00319/2024-04-30/2024-04-30/text/original/epub/OEBPS/document_1/document_1.html#_Toc166158182> ;
    dcat:landingPage "https://www.legislation.gov.au/F2021L00319/2024-04-30/2024-04-30/text/original/epub/OEBPS/document_1/document_1.html#_Toc166158182"^^xsd:anyURI ;
    dcat:theme legcons:Item .

F2021L00319:352 a legcons:Item,
        owl:Class,
        dcat:Resource ;
    rdfs:label "Item - I352 11 1  Reviewable decisions"@en-AU ;
    dct:isPartOf F2021L00319:351 ;
    dct:isReferencedBy F2021L00319: ;
    rdfs:comment "11 1  Reviewable decisions - Abrievated Graph Key: I352"@en-AU ;
    skos:definition "11 1  Reviewable decisions"@en-AU ;
    skos:narrower F2021L00319:351 ;
    skos:prefLabel "Item I352"@en-AU ;
    dcat:accessURL <https://www.legislation.gov.au/F2021L00319/2024-04-30/2024-04-30/text/original/epub/OEBPS/document_1/document_1.html#_Toc166158185> ;
    dcat:landingPage "https://www.legislation.gov.au/F2021L00319/2024-04-30/2024-04-30/text/original/epub/OEBPS/document_1/document_1.html#_Toc166158185"^^xsd:anyURI ;
    dcat:theme legcons:Item .

F2021L00319:354 a legcons:Item,
        owl:Class,
        dcat:Resource ;
    rdfs:label "Item - I354 11 2  Purpose of this Part"@en-AU ;
    dct:isPartOf F2021L00319:353 ;
    dct:isReferencedBy F2021L00319: ;
    rdfs:comment "11 2  Purpose of this Part - Abrievated Graph Key: I354"@en-AU ;
    skos:definition "11 2  Purpose of this Part"@en-AU ;
    skos:narrower F2021L00319:353 ;
    skos:prefLabel "Item I354"@en-AU ;
    dcat:accessURL <https://www.legislation.gov.au/F2021L00319/2024-04-30/2024-04-30/text/original/epub/OEBPS/document_1/document_1.html#_Toc166158187> ;
    dcat:landingPage "https://www.legislation.gov.au/F2021L00319/2024-04-30/2024-04-30/text/original/epub/OEBPS/document_1/document_1.html#_Toc166158187"^^xsd:anyURI ;
    dcat:theme legcons:Item .

F2021L00319:355 a legcons:Item,
        owl:Class,
        dcat:Resource ;
    rdfs:label "Item - I355 11 3  General requirements for records"@en-AU ;
    dct:isPartOf F2021L00319:353 ;
    dct:isReferencedBy F2021L00319: ;
    rdfs:comment "11 3  General requirements for records - Abrievated Graph Key: I355"@en-AU ;
    skos:definition "11 3  General requirements for records"@en-AU ;
    skos:narrower F2021L00319:353 ;
    skos:prefLabel "Item I355"@en-AU ;
    dcat:accessURL <https://www.legislation.gov.au/F2021L00319/2024-04-30/2024-04-30/text/original/epub/OEBPS/document_1/document_1.html#_Toc166158188> ;
    dcat:landingPage "https://www.legislation.gov.au/F2021L00319/2024-04-30/2024-04-30/text/original/epub/OEBPS/document_1/document_1.html#_Toc166158188"^^xsd:anyURI ;
    dcat:theme legcons:Item .

F2021L00319:356 a legcons:Item,
        owl:Class,
        dcat:Resource ;
    rdfs:label "Item - I356 11 4  Government certificates"@en-AU ;
    dct:isPartOf F2021L00319:353 ;
    dct:isReferencedBy F2021L00319: ;
    rdfs:comment "11 4  Government certificates - Abrievated Graph Key: I356"@en-AU ;
    skos:definition "11 4  Government certificates"@en-AU ;
    skos:narrower F2021L00319:353 ;
    skos:prefLabel "Item I356"@en-AU ;
    dcat:accessURL <https://www.legislation.gov.au/F2021L00319/2024-04-30/2024-04-30/text/original/epub/OEBPS/document_1/document_1.html#_Toc166158189> ;
    dcat:landingPage "https://www.legislation.gov.au/F2021L00319/2024-04-30/2024-04-30/text/original/epub/OEBPS/document_1/document_1.html#_Toc166158189"^^xsd:anyURI ;
    dcat:theme legcons:Item .

F2021L00319:357 a legcons:Item,
        owl:Class,
        dcat:Resource ;
    rdfs:label "Item - I357 11 5  Export permits"@en-AU ;
    dct:isPartOf F2021L00319:353 ;
    dct:isReferencedBy F2021L00319: ;
    rdfs:comment "11 5  Export permits - Abrievated Graph Key: I357"@en-AU ;
    skos:definition "11 5  Export permits"@en-AU ;
    skos:narrower F2021L00319:353 ;
    skos:prefLabel "Item I357"@en-AU ;
    dcat:accessURL <https://www.legislation.gov.au/F2021L00319/2024-04-30/2024-04-30/text/original/epub/OEBPS/document_1/document_1.html#_Toc166158190> ;
    dcat:landingPage "https://www.legislation.gov.au/F2021L00319/2024-04-30/2024-04-30/text/original/epub/OEBPS/document_1/document_1.html#_Toc166158190"^^xsd:anyURI ;
    dcat:theme legcons:Item .

F2021L00319:358 a legcons:Item,
        owl:Class,
        dcat:Resource ;
    rdfs:label "Item - I358 11 6  Records to be retained by exporter"@en-AU ;
    dct:isPartOf F2021L00319:353 ;
    dct:isReferencedBy F2021L00319: ;
    rdfs:comment "11 6  Records to be retained by exporter - Abrievated Graph Key: I358"@en-AU ;
    skos:definition "11 6  Records to be retained by exporter"@en-AU ;
    skos:narrower F2021L00319:353 ;
    skos:prefLabel "Item I358"@en-AU ;
    dcat:accessURL <https://www.legislation.gov.au/F2021L00319/2024-04-30/2024-04-30/text/original/epub/OEBPS/document_1/document_1.html#_Toc166158191> ;
    dcat:landingPage "https://www.legislation.gov.au/F2021L00319/2024-04-30/2024-04-30/text/original/epub/OEBPS/document_1/document_1.html#_Toc166158191"^^xsd:anyURI ;
    dcat:theme legcons:Item .

F2021L00319:359 a legcons:Item,
        owl:Class,
        dcat:Resource ;
    rdfs:label "Item - I359 11 7  Records to be retained by occupier of registered establishment"@en-AU ;
    dct:isPartOf F2021L00319:353 ;
    dct:isReferencedBy F2021L00319: ;
    rdfs:comment "11 7  Records to be retained by occupier of registered establishment - Abrievated Graph Key: I359"@en-AU ;
    skos:definition "11 7  Records to be retained by occupier of registered establishment"@en-AU ;
    skos:narrower F2021L00319:353 ;
    skos:prefLabel "Item I359"@en-AU ;
    dcat:accessURL <https://www.legislation.gov.au/F2021L00319/2024-04-30/2024-04-30/text/original/epub/OEBPS/document_1/document_1.html#_Toc166158192> ;
    dcat:landingPage "https://www.legislation.gov.au/F2021L00319/2024-04-30/2024-04-30/text/original/epub/OEBPS/document_1/document_1.html#_Toc166158192"^^xsd:anyURI ;
    dcat:theme legcons:Item .

F2021L00319:36 a legcons:Item,
        owl:Class,
        dcat:Resource ;
    rdfs:label "Item - I36 2 18  Application of this Division"@en-AU ;
    dct:isPartOf F2021L00319:35 ;
    dct:isReferencedBy F2021L00319: ;
    rdfs:comment "2 18  Application of this Division - Abrievated Graph Key: I36"@en-AU ;
    skos:definition "2 18  Application of this Division"@en-AU ;
    skos:narrower F2021L00319:35 ;
    skos:prefLabel "Item I36"@en-AU ;
    dcat:accessURL <https://www.legislation.gov.au/F2021L00319/2024-04-30/2024-04-30/text/original/epub/OEBPS/document_1/document_1.html#_Toc166157869> ;
    dcat:landingPage "https://www.legislation.gov.au/F2021L00319/2024-04-30/2024-04-30/text/original/epub/OEBPS/document_1/document_1.html#_Toc166157869"^^xsd:anyURI ;
    dcat:theme legcons:Item .

F2021L00319:360 a legcons:Item,
        owl:Class,
        dcat:Resource ;
    rdfs:label "Item - I360 11 8  Records to be retained by holder of approved arrangement"@en-AU ;
    dct:isPartOf F2021L00319:353 ;
    dct:isReferencedBy F2021L00319: ;
    rdfs:comment "11 8  Records to be retained by holder of approved arrangement - Abrievated Graph Key: I360"@en-AU ;
    skos:definition "11 8  Records to be retained by holder of approved arrangement"@en-AU ;
    skos:narrower F2021L00319:353 ;
    skos:prefLabel "Item I360"@en-AU ;
    dcat:accessURL <https://www.legislation.gov.au/F2021L00319/2024-04-30/2024-04-30/text/original/epub/OEBPS/document_1/document_1.html#_Toc166158193> ;
    dcat:landingPage "https://www.legislation.gov.au/F2021L00319/2024-04-30/2024-04-30/text/original/epub/OEBPS/document_1/document_1.html#_Toc166158193"^^xsd:anyURI ;
    dcat:theme legcons:Item .

F2021L00319:361 a legcons:Item,
        owl:Class,
        dcat:Resource ;
    rdfs:label "Item - I361 11 9  Records relating to official marks"@en-AU ;
    dct:isPartOf F2021L00319:353 ;
    dct:isReferencedBy F2021L00319: ;
    rdfs:comment "11 9  Records relating to official marks - Abrievated Graph Key: I361"@en-AU ;
    skos:definition "11 9  Records relating to official marks"@en-AU ;
    skos:narrower F2021L00319:353 ;
    skos:prefLabel "Item I361"@en-AU ;
    dcat:accessURL <https://www.legislation.gov.au/F2021L00319/2024-04-30/2024-04-30/text/original/epub/OEBPS/document_1/document_1.html#_Toc166158194> ;
    dcat:landingPage "https://www.legislation.gov.au/F2021L00319/2024-04-30/2024-04-30/text/original/epub/OEBPS/document_1/document_1.html#_Toc166158194"^^xsd:anyURI ;
    dcat:theme legcons:Item .

F2021L00319:362 a legcons:Item,
        owl:Class,
        dcat:Resource ;
    rdfs:label "Item - I362 11 10  Records relating to official marking devices"@en-AU ;
    dct:isPartOf F2021L00319:353 ;
    dct:isReferencedBy F2021L00319: ;
    rdfs:comment "11 10  Records relating to official marking devices - Abrievated Graph Key: I362"@en-AU ;
    skos:definition "11 10  Records relating to official marking devices"@en-AU ;
    skos:narrower F2021L00319:353 ;
    skos:prefLabel "Item I362"@en-AU ;
    dcat:accessURL <https://www.legislation.gov.au/F2021L00319/2024-04-30/2024-04-30/text/original/epub/OEBPS/document_1/document_1.html#_Toc166158195> ;
    dcat:landingPage "https://www.legislation.gov.au/F2021L00319/2024-04-30/2024-04-30/text/original/epub/OEBPS/document_1/document_1.html#_Toc166158195"^^xsd:anyURI ;
    dcat:theme legcons:Item .

F2021L00319:363 a legcons:Item,
        owl:Class,
        dcat:Resource ;
    rdfs:label "Item - I363 11 11  Records must not be altered or defaced during retention period"@en-AU ;
    dct:isPartOf F2021L00319:353 ;
    dct:isReferencedBy F2021L00319: ;
    rdfs:comment "11 11  Records must not be altered or defaced during retention period - Abrievated Graph Key: I363"@en-AU ;
    skos:definition "11 11  Records must not be altered or defaced during retention period"@en-AU ;
    skos:narrower F2021L00319:353 ;
    skos:prefLabel "Item I363"@en-AU ;
    dcat:accessURL <https://www.legislation.gov.au/F2021L00319/2024-04-30/2024-04-30/text/original/epub/OEBPS/document_1/document_1.html#_Toc166158196> ;
    dcat:landingPage "https://www.legislation.gov.au/F2021L00319/2024-04-30/2024-04-30/text/original/epub/OEBPS/document_1/document_1.html#_Toc166158196"^^xsd:anyURI ;
    dcat:theme legcons:Item .

F2021L00319:365 a legcons:Item,
        owl:Class,
        dcat:Resource ;
    rdfs:label "Item - I365 11 12  Storage of samples"@en-AU ;
    dct:isPartOf F2021L00319:364 ;
    dct:isReferencedBy F2021L00319: ;
    rdfs:comment "11 12  Storage of samples - Abrievated Graph Key: I365"@en-AU ;
    skos:definition "11 12  Storage of samples"@en-AU ;
    skos:narrower F2021L00319:364 ;
    skos:prefLabel "Item I365"@en-AU ;
    dcat:accessURL <https://www.legislation.gov.au/F2021L00319/2024-04-30/2024-04-30/text/original/epub/OEBPS/document_1/document_1.html#_Toc166158198> ;
    dcat:landingPage "https://www.legislation.gov.au/F2021L00319/2024-04-30/2024-04-30/text/original/epub/OEBPS/document_1/document_1.html#_Toc166158198"^^xsd:anyURI ;
    dcat:theme legcons:Item .

F2021L00319:367 a legcons:Item,
        owl:Class,
        dcat:Resource ;
    rdfs:label "Item - I367 11 13  Division of compensation between owners"@en-AU ;
    dct:isPartOf F2021L00319:366 ;
    dct:isReferencedBy F2021L00319: ;
    rdfs:comment "11 13  Division of compensation between owners - Abrievated Graph Key: I367"@en-AU ;
    skos:definition "11 13  Division of compensation between owners"@en-AU ;
    skos:narrower F2021L00319:366 ;
    skos:prefLabel "Item I367"@en-AU ;
    dcat:accessURL <https://www.legislation.gov.au/F2021L00319/2024-04-30/2024-04-30/text/original/epub/OEBPS/document_1/document_1.html#_Toc166158200> ;
    dcat:landingPage "https://www.legislation.gov.au/F2021L00319/2024-04-30/2024-04-30/text/original/epub/OEBPS/document_1/document_1.html#_Toc166158200"^^xsd:anyURI ;
    dcat:theme legcons:Item .

F2021L00319:368 a legcons:Item,
        owl:Class,
        dcat:Resource ;
    rdfs:label "Item - I368 11 14  Amount of compensation"@en-AU ;
    dct:isPartOf F2021L00319:366 ;
    dct:isReferencedBy F2021L00319: ;
    rdfs:comment "11 14  Amount of compensation - Abrievated Graph Key: I368"@en-AU ;
    skos:definition "11 14  Amount of compensation"@en-AU ;
    skos:narrower F2021L00319:366 ;
    skos:prefLabel "Item I368"@en-AU ;
    dcat:accessURL <https://www.legislation.gov.au/F2021L00319/2024-04-30/2024-04-30/text/original/epub/OEBPS/document_1/document_1.html#_Toc166158201> ;
    dcat:landingPage "https://www.legislation.gov.au/F2021L00319/2024-04-30/2024-04-30/text/original/epub/OEBPS/document_1/document_1.html#_Toc166158201"^^xsd:anyURI ;
    dcat:theme legcons:Item .

F2021L00319:37 a legcons:Item,
        owl:Class,
        dcat:Resource ;
    rdfs:label "Item - I37 2 19  When application for government certificate may be made"@en-AU ;
    dct:isPartOf F2021L00319:35 ;
    dct:isReferencedBy F2021L00319: ;
    rdfs:comment "2 19  When application for government certificate may be made - Abrievated Graph Key: I37"@en-AU ;
    skos:definition "2 19  When application for government certificate may be made"@en-AU ;
    skos:narrower F2021L00319:35 ;
    skos:prefLabel "Item I37"@en-AU ;
    dcat:accessURL <https://www.legislation.gov.au/F2021L00319/2024-04-30/2024-04-30/text/original/epub/OEBPS/document_1/document_1.html#_Toc166157870> ;
    dcat:landingPage "https://www.legislation.gov.au/F2021L00319/2024-04-30/2024-04-30/text/original/epub/OEBPS/document_1/document_1.html#_Toc166157870"^^xsd:anyURI ;
    dcat:theme legcons:Item .

F2021L00319:370 a legcons:Item,
        owl:Class,
        dcat:Resource ;
    rdfs:label "Item - I370 11 15  Circumstances in which relevant Commonwealth liability of a person is taken to have been paid"@en-AU ;
    dct:isPartOf F2021L00319:369 ;
    dct:isReferencedBy F2021L00319: ;
    rdfs:comment "11 15  Circumstances in which relevant Commonwealth liability of a person is taken to have been paid - Abrievated Graph Key: I370"@en-AU ;
    skos:definition "11 15  Circumstances in which relevant Commonwealth liability of a person is taken to have been paid"@en-AU ;
    skos:narrower F2021L00319:369 ;
    skos:prefLabel "Item I370"@en-AU ;
    dcat:accessURL <https://www.legislation.gov.au/F2021L00319/2024-04-30/2024-04-30/text/original/epub/OEBPS/document_1/document_1.html#_Toc166158203> ;
    dcat:landingPage "https://www.legislation.gov.au/F2021L00319/2024-04-30/2024-04-30/text/original/epub/OEBPS/document_1/document_1.html#_Toc166158203"^^xsd:anyURI ;
    dcat:theme legcons:Item .

F2021L00319:372 a legcons:Item,
        owl:Class,
        dcat:Resource ;
    rdfs:label "Item - I372 11 16  Collection of information from agriculture regulators"@en-AU ;
    dct:isPartOf F2021L00319:371 ;
    dct:isReferencedBy F2021L00319: ;
    rdfs:comment "11 16  Collection of information from agriculture regulators - Abrievated Graph Key: I372"@en-AU ;
    skos:definition "11 16  Collection of information from agriculture regulators"@en-AU ;
    skos:narrower F2021L00319:371 ;
    skos:prefLabel "Item I372"@en-AU ;
    dcat:accessURL <https://www.legislation.gov.au/F2021L00319/2024-04-30/2024-04-30/text/original/epub/OEBPS/document_1/document_1.html#_Toc166158205> ;
    dcat:landingPage "https://www.legislation.gov.au/F2021L00319/2024-04-30/2024-04-30/text/original/epub/OEBPS/document_1/document_1.html#_Toc166158205"^^xsd:anyURI ;
    dcat:theme legcons:Item .

F2021L00319:375 a legcons:Item,
        owl:Class,
        dcat:Resource ;
    rdfs:label "Item - I375 12 1  Definitions"@en-AU ;
    dct:isPartOf F2021L00319:374 ;
    dct:isReferencedBy F2021L00319: ;
    rdfs:comment "12 1  Definitions - Abrievated Graph Key: I375"@en-AU ;
    skos:definition "12 1  Definitions"@en-AU ;
    skos:narrower F2021L00319:374 ;
    skos:prefLabel "Item I375"@en-AU ;
    dcat:accessURL <https://www.legislation.gov.au/F2021L00319/2024-04-30/2024-04-30/text/original/epub/OEBPS/document_1/document_1.html#_Toc166158208> ;
    dcat:landingPage "https://www.legislation.gov.au/F2021L00319/2024-04-30/2024-04-30/text/original/epub/OEBPS/document_1/document_1.html#_Toc166158208"^^xsd:anyURI ;
    dcat:theme legcons:Item .

F2021L00319:377 a legcons:Item,
        owl:Class,
        dcat:Resource ;
    rdfs:label "Item - I377 12 2  Application to alter operations manual made but not decided before commencement time"@en-AU ;
    dct:isPartOf F2021L00319:376 ;
    dct:isReferencedBy F2021L00319: ;
    rdfs:comment "12 2  Application to alter operations manual made but not decided before commencement time - Abrievated Graph Key: I377"@en-AU ;
    skos:definition "12 2  Application to alter operations manual made but not decided before commencement time"@en-AU ;
    skos:narrower F2021L00319:376 ;
    skos:prefLabel "Item I377"@en-AU ;
    dcat:accessURL <https://www.legislation.gov.au/F2021L00319/2024-04-30/2024-04-30/text/original/epub/OEBPS/document_1/document_1.html#_Toc166158210> ;
    dcat:landingPage "https://www.legislation.gov.au/F2021L00319/2024-04-30/2024-04-30/text/original/epub/OEBPS/document_1/document_1.html#_Toc166158210"^^xsd:anyURI ;
    dcat:theme legcons:Item .

F2021L00319:378 a legcons:Item,
        owl:Class,
        dcat:Resource ;
    rdfs:label "Item - I378 12 3  Direction given to operator of registered premises before commencement time to alter operations manual"@en-AU ;
    dct:isPartOf F2021L00319:376 ;
    dct:isReferencedBy F2021L00319: ;
    rdfs:comment "12 3  Direction given to operator of registered premises before commencement time to alter operations manual - Abrievated Graph Key: I378"@en-AU ;
    skos:definition "12 3  Direction given to operator of registered premises before commencement time to alter operations manual"@en-AU ;
    skos:narrower F2021L00319:376 ;
    skos:prefLabel "Item I378"@en-AU ;
    dcat:accessURL <https://www.legislation.gov.au/F2021L00319/2024-04-30/2024-04-30/text/original/epub/OEBPS/document_1/document_1.html#_Toc166158211> ;
    dcat:landingPage "https://www.legislation.gov.au/F2021L00319/2024-04-30/2024-04-30/text/original/epub/OEBPS/document_1/document_1.html#_Toc166158211"^^xsd:anyURI ;
    dcat:theme legcons:Item .

F2021L00319:38 a legcons:Item,
        owl:Class,
        dcat:Resource ;
    rdfs:label "Item - I38 2 21  Requirements that must be complied with before government certificate may be issued"@en-AU ;
    dct:isPartOf F2021L00319:35 ;
    dct:isReferencedBy F2021L00319: ;
    rdfs:comment "2 21  Requirements that must be complied with before government certificate may be issued - Abrievated Graph Key: I38"@en-AU ;
    skos:definition "2 21  Requirements that must be complied with before government certificate may be issued"@en-AU ;
    skos:narrower F2021L00319:35 ;
    skos:prefLabel "Item I38"@en-AU ;
    dcat:accessURL <https://www.legislation.gov.au/F2021L00319/2024-04-30/2024-04-30/text/original/epub/OEBPS/document_1/document_1.html#_Toc166157871> ;
    dcat:landingPage "https://www.legislation.gov.au/F2021L00319/2024-04-30/2024-04-30/text/original/epub/OEBPS/document_1/document_1.html#_Toc166157871"^^xsd:anyURI ;
    dcat:theme legcons:Item .

F2021L00319:380 a legcons:Item,
        owl:Class,
        dcat:Resource ;
    rdfs:label "Item - I380 12 4  ESCAS approved before commencement time"@en-AU ;
    dct:isPartOf F2021L00319:379 ;
    dct:isReferencedBy F2021L00319: ;
    rdfs:comment "12 4  ESCAS approved before commencement time - Abrievated Graph Key: I380"@en-AU ;
    skos:definition "12 4  ESCAS approved before commencement time"@en-AU ;
    skos:narrower F2021L00319:379 ;
    skos:prefLabel "Item I380"@en-AU ;
    dcat:accessURL <https://www.legislation.gov.au/F2021L00319/2024-04-30/2024-04-30/text/original/epub/OEBPS/document_1/document_1.html#_Toc166158213> ;
    dcat:landingPage "https://www.legislation.gov.au/F2021L00319/2024-04-30/2024-04-30/text/original/epub/OEBPS/document_1/document_1.html#_Toc166158213"^^xsd:anyURI ;
    dcat:theme legcons:Item .

F2021L00319:381 a legcons:Item,
        owl:Class,
        dcat:Resource ;
    rdfs:label "Item - I381 12 5  Request to vary ESCAS made before commencement time"@en-AU ;
    dct:isPartOf F2021L00319:379 ;
    dct:isReferencedBy F2021L00319: ;
    rdfs:comment "12 5  Request to vary ESCAS made before commencement time - Abrievated Graph Key: I381"@en-AU ;
    skos:definition "12 5  Request to vary ESCAS made before commencement time"@en-AU ;
    skos:narrower F2021L00319:379 ;
    skos:prefLabel "Item I381"@en-AU ;
    dcat:accessURL <https://www.legislation.gov.au/F2021L00319/2024-04-30/2024-04-30/text/original/epub/OEBPS/document_1/document_1.html#_Toc166158214> ;
    dcat:landingPage "https://www.legislation.gov.au/F2021L00319/2024-04-30/2024-04-30/text/original/epub/OEBPS/document_1/document_1.html#_Toc166158214"^^xsd:anyURI ;
    dcat:theme legcons:Item .

F2021L00319:382 a legcons:Item,
        owl:Class,
        dcat:Resource ;
    rdfs:label "Item - I382 12 6  Variation of approved ESCAS required by Secretary before commencement time"@en-AU ;
    dct:isPartOf F2021L00319:379 ;
    dct:isReferencedBy F2021L00319: ;
    rdfs:comment "12 6  Variation of approved ESCAS required by Secretary before commencement time - Abrievated Graph Key: I382"@en-AU ;
    skos:definition "12 6  Variation of approved ESCAS required by Secretary before commencement time"@en-AU ;
    skos:narrower F2021L00319:379 ;
    skos:prefLabel "Item I382"@en-AU ;
    dcat:accessURL <https://www.legislation.gov.au/F2021L00319/2024-04-30/2024-04-30/text/original/epub/OEBPS/document_1/document_1.html#_Toc166158215> ;
    dcat:landingPage "https://www.legislation.gov.au/F2021L00319/2024-04-30/2024-04-30/text/original/epub/OEBPS/document_1/document_1.html#_Toc166158215"^^xsd:anyURI ;
    dcat:theme legcons:Item .

F2021L00319:385 a legcons:Item,
        owl:Class,
        dcat:Resource ;
    rdfs:label "Item - I385 12 7  Notice of intention to export consignment of livestock approved but consignment not exported before commencement time"@en-AU ;
    dct:isPartOf F2021L00319:384 ;
    dct:isReferencedBy F2021L00319: ;
    rdfs:comment "12 7  Notice of intention to export consignment of livestock approved but consignment not exported before commencement time - Abrievated Graph Key: I385"@en-AU ;
    skos:definition "12 7  Notice of intention to export consignment of livestock approved but consignment not exported before commencement time"@en-AU ;
    skos:narrower F2021L00319:384 ;
    skos:prefLabel "Item I385"@en-AU ;
    dcat:accessURL <https://www.legislation.gov.au/F2021L00319/2024-04-30/2024-04-30/text/original/epub/OEBPS/document_1/document_1.html#_Toc166158218> ;
    dcat:landingPage "https://www.legislation.gov.au/F2021L00319/2024-04-30/2024-04-30/text/original/epub/OEBPS/document_1/document_1.html#_Toc166158218"^^xsd:anyURI ;
    dcat:theme legcons:Item .

F2021L00319:386 a legcons:Item,
        owl:Class,
        dcat:Resource ;
    rdfs:label "Item - I386 12 8  Approval of premises for pre export quarantine or isolation of consignment of livestock given before commencement time"@en-AU ;
    dct:isPartOf F2021L00319:384 ;
    dct:isReferencedBy F2021L00319: ;
    rdfs:comment "12 8  Approval of premises for pre export quarantine or isolation of consignment of livestock given before commencement time - Abrievated Graph Key: I386"@en-AU ;
    skos:definition "12 8  Approval of premises for pre export quarantine or isolation of consignment of livestock given before commencement time"@en-AU ;
    skos:narrower F2021L00319:384 ;
    skos:prefLabel "Item I386"@en-AU ;
    dcat:accessURL <https://www.legislation.gov.au/F2021L00319/2024-04-30/2024-04-30/text/original/epub/OEBPS/document_1/document_1.html#_Toc166158219> ;
    dcat:landingPage "https://www.legislation.gov.au/F2021L00319/2024-04-30/2024-04-30/text/original/epub/OEBPS/document_1/document_1.html#_Toc166158219"^^xsd:anyURI ;
    dcat:theme legcons:Item .

F2021L00319:387 a legcons:Item,
        owl:Class,
        dcat:Resource ;
    rdfs:label "Item - I387 12 9  Notice of intention to export consignment of live animals approved but consignment not exported before commencement time"@en-AU ;
    dct:isPartOf F2021L00319:384 ;
    dct:isReferencedBy F2021L00319: ;
    rdfs:comment "12 9  Notice of intention to export consignment of live animals approved but consignment not exported before commencement time - Abrievated Graph Key: I387"@en-AU ;
    skos:definition "12 9  Notice of intention to export consignment of live animals approved but consignment not exported before commencement time"@en-AU ;
    skos:narrower F2021L00319:384 ;
    skos:prefLabel "Item I387"@en-AU ;
    dcat:accessURL <https://www.legislation.gov.au/F2021L00319/2024-04-30/2024-04-30/text/original/epub/OEBPS/document_1/document_1.html#_Toc166158220> ;
    dcat:landingPage "https://www.legislation.gov.au/F2021L00319/2024-04-30/2024-04-30/text/original/epub/OEBPS/document_1/document_1.html#_Toc166158220"^^xsd:anyURI ;
    dcat:theme legcons:Item .

F2021L00319:388 a legcons:Item,
        owl:Class,
        dcat:Resource ;
    rdfs:label "Item - I388 12 10  Approval of premises for pre export quarantine or isolation of consignment of live animals given before commencement time"@en-AU ;
    dct:isPartOf F2021L00319:384 ;
    dct:isReferencedBy F2021L00319: ;
    rdfs:comment "12 10  Approval of premises for pre export quarantine or isolation of consignment of live animals given before commencement time - Abrievated Graph Key: I388"@en-AU ;
    skos:definition "12 10  Approval of premises for pre export quarantine or isolation of consignment of live animals given before commencement time"@en-AU ;
    skos:narrower F2021L00319:384 ;
    skos:prefLabel "Item I388"@en-AU ;
    dcat:accessURL <https://www.legislation.gov.au/F2021L00319/2024-04-30/2024-04-30/text/original/epub/OEBPS/document_1/document_1.html#_Toc166158221> ;
    dcat:landingPage "https://www.legislation.gov.au/F2021L00319/2024-04-30/2024-04-30/text/original/epub/OEBPS/document_1/document_1.html#_Toc166158221"^^xsd:anyURI ;
    dcat:theme legcons:Item .

F2021L00319:39 a legcons:Item,
        owl:Class,
        dcat:Resource ;
    rdfs:label "Item - I39 2 22  Issuing body must consider conditions if any of approval of notice of intention to export consignment"@en-AU ;
    dct:isPartOf F2021L00319:35 ;
    dct:isReferencedBy F2021L00319: ;
    rdfs:comment "2 22  Issuing body must consider conditions if any of approval of notice of intention to export consignment - Abrievated Graph Key: I39"@en-AU ;
    skos:definition "2 22  Issuing body must consider conditions if any of approval of notice of intention to export consignment"@en-AU ;
    skos:narrower F2021L00319:35 ;
    skos:prefLabel "Item I39"@en-AU ;
    dcat:accessURL <https://www.legislation.gov.au/F2021L00319/2024-04-30/2024-04-30/text/original/epub/OEBPS/document_1/document_1.html#_Toc166157872> ;
    dcat:landingPage "https://www.legislation.gov.au/F2021L00319/2024-04-30/2024-04-30/text/original/epub/OEBPS/document_1/document_1.html#_Toc166157872"^^xsd:anyURI ;
    dcat:theme legcons:Item .

F2021L00319:390 a legcons:Item,
        owl:Class,
        dcat:Resource ;
    rdfs:label "Item - I390 12 11  Person approved before commencement time to manufacture an official mark"@en-AU ;
    dct:isPartOf F2021L00319:389 ;
    dct:isReferencedBy F2021L00319: ;
    rdfs:comment "12 11  Person approved before commencement time to manufacture an official mark - Abrievated Graph Key: I390"@en-AU ;
    skos:definition "12 11  Person approved before commencement time to manufacture an official mark"@en-AU ;
    skos:narrower F2021L00319:389 ;
    skos:prefLabel "Item I390"@en-AU ;
    dcat:accessURL <https://www.legislation.gov.au/F2021L00319/2024-04-30/2024-04-30/text/original/epub/OEBPS/document_1/document_1.html#_Toc166158223> ;
    dcat:landingPage "https://www.legislation.gov.au/F2021L00319/2024-04-30/2024-04-30/text/original/epub/OEBPS/document_1/document_1.html#_Toc166158223"^^xsd:anyURI ;
    dcat:theme legcons:Item .

F2021L00319:391 a legcons:Item,
        owl:Class,
        dcat:Resource ;
    rdfs:label "Item - I391 12 12  Person approved before commencement time to possess an official mark"@en-AU ;
    dct:isPartOf F2021L00319:389 ;
    dct:isReferencedBy F2021L00319: ;
    rdfs:comment "12 12  Person approved before commencement time to possess an official mark - Abrievated Graph Key: I391"@en-AU ;
    skos:definition "12 12  Person approved before commencement time to possess an official mark"@en-AU ;
    skos:narrower F2021L00319:389 ;
    skos:prefLabel "Item I391"@en-AU ;
    dcat:accessURL <https://www.legislation.gov.au/F2021L00319/2024-04-30/2024-04-30/text/original/epub/OEBPS/document_1/document_1.html#_Toc166158224> ;
    dcat:landingPage "https://www.legislation.gov.au/F2021L00319/2024-04-30/2024-04-30/text/original/epub/OEBPS/document_1/document_1.html#_Toc166158224"^^xsd:anyURI ;
    dcat:theme legcons:Item .

F2021L00319:392 a legcons:Item,
        owl:Class,
        dcat:Resource ;
    rdfs:label "Item - I392 12 13  Person approved before commencement time to apply an official mark"@en-AU ;
    dct:isPartOf F2021L00319:389 ;
    dct:isReferencedBy F2021L00319: ;
    rdfs:comment "12 13  Person approved before commencement time to apply an official mark - Abrievated Graph Key: I392"@en-AU ;
    skos:definition "12 13  Person approved before commencement time to apply an official mark"@en-AU ;
    skos:narrower F2021L00319:389 ;
    skos:prefLabel "Item I392"@en-AU ;
    dcat:accessURL <https://www.legislation.gov.au/F2021L00319/2024-04-30/2024-04-30/text/original/epub/OEBPS/document_1/document_1.html#_Toc166158225> ;
    dcat:landingPage "https://www.legislation.gov.au/F2021L00319/2024-04-30/2024-04-30/text/original/epub/OEBPS/document_1/document_1.html#_Toc166158225"^^xsd:anyURI ;
    dcat:theme legcons:Item .

F2021L00319:394 a legcons:Item,
        owl:Class,
        dcat:Resource ;
    rdfs:label "Item - I394 12 14  Person approved before commencement time to manufacture an official marking device"@en-AU ;
    dct:isPartOf F2021L00319:393 ;
    dct:isReferencedBy F2021L00319: ;
    rdfs:comment "12 14  Person approved before commencement time to manufacture an official marking device - Abrievated Graph Key: I394"@en-AU ;
    skos:definition "12 14  Person approved before commencement time to manufacture an official marking device"@en-AU ;
    skos:narrower F2021L00319:393 ;
    skos:prefLabel "Item I394"@en-AU ;
    dcat:accessURL <https://www.legislation.gov.au/F2021L00319/2024-04-30/2024-04-30/text/original/epub/OEBPS/document_1/document_1.html#_Toc166158227> ;
    dcat:landingPage "https://www.legislation.gov.au/F2021L00319/2024-04-30/2024-04-30/text/original/epub/OEBPS/document_1/document_1.html#_Toc166158227"^^xsd:anyURI ;
    dcat:theme legcons:Item .

F2021L00319:395 a legcons:Item,
        owl:Class,
        dcat:Resource ;
    rdfs:label "Item - I395 12 15  Person approved before commencement time to possess an official marking device"@en-AU ;
    dct:isPartOf F2021L00319:393 ;
    dct:isReferencedBy F2021L00319: ;
    rdfs:comment "12 15  Person approved before commencement time to possess an official marking device - Abrievated Graph Key: I395"@en-AU ;
    skos:definition "12 15  Person approved before commencement time to possess an official marking device"@en-AU ;
    skos:narrower F2021L00319:393 ;
    skos:prefLabel "Item I395"@en-AU ;
    dcat:accessURL <https://www.legislation.gov.au/F2021L00319/2024-04-30/2024-04-30/text/original/epub/OEBPS/document_1/document_1.html#_Toc166158228> ;
    dcat:landingPage "https://www.legislation.gov.au/F2021L00319/2024-04-30/2024-04-30/text/original/epub/OEBPS/document_1/document_1.html#_Toc166158228"^^xsd:anyURI ;
    dcat:theme legcons:Item .

F2021L00319:398 a legcons:Item,
        owl:Class,
        dcat:Resource ;
    rdfs:label "Item - I398 12 16  Accreditations of veterinarians in force immediately before commencement time"@en-AU ;
    dct:isPartOf F2021L00319:397 ;
    dct:isReferencedBy F2021L00319: ;
    rdfs:comment "12 16  Accreditations of veterinarians in force immediately before commencement time - Abrievated Graph Key: I398"@en-AU ;
    skos:definition "12 16  Accreditations of veterinarians in force immediately before commencement time"@en-AU ;
    skos:narrower F2021L00319:397 ;
    skos:prefLabel "Item I398"@en-AU ;
    dcat:accessURL <https://www.legislation.gov.au/F2021L00319/2024-04-30/2024-04-30/text/original/epub/OEBPS/document_1/document_1.html#_Toc166158231> ;
    dcat:landingPage "https://www.legislation.gov.au/F2021L00319/2024-04-30/2024-04-30/text/original/epub/OEBPS/document_1/document_1.html#_Toc166158231"^^xsd:anyURI ;
    dcat:theme legcons:Item .

F2021L00319:399 a legcons:Item,
        owl:Class,
        dcat:Resource ;
    rdfs:label "Item - I399 12 17  Application for accreditation of veterinarian made but not decided before commencement time"@en-AU ;
    dct:isPartOf F2021L00319:397 ;
    dct:isReferencedBy F2021L00319: ;
    rdfs:comment "12 17  Application for accreditation of veterinarian made but not decided before commencement time - Abrievated Graph Key: I399"@en-AU ;
    skos:definition "12 17  Application for accreditation of veterinarian made but not decided before commencement time"@en-AU ;
    skos:narrower F2021L00319:397 ;
    skos:prefLabel "Item I399"@en-AU ;
    dcat:accessURL <https://www.legislation.gov.au/F2021L00319/2024-04-30/2024-04-30/text/original/epub/OEBPS/document_1/document_1.html#_Toc166158232> ;
    dcat:landingPage "https://www.legislation.gov.au/F2021L00319/2024-04-30/2024-04-30/text/original/epub/OEBPS/document_1/document_1.html#_Toc166158232"^^xsd:anyURI ;
    dcat:theme legcons:Item .

F2021L00319:4 a legcons:Item,
        owl:Class,
        dcat:Resource ;
    rdfs:label "Item - I4 1 3  Authority"@en-AU ;
    dct:isPartOf F2021L00319:1 ;
    dct:isReferencedBy F2021L00319: ;
    rdfs:comment "1 3  Authority - Abrievated Graph Key: I4"@en-AU ;
    skos:definition "1 3  Authority"@en-AU ;
    skos:narrower F2021L00319:1 ;
    skos:prefLabel "Item I4"@en-AU ;
    dcat:accessURL <https://www.legislation.gov.au/F2021L00319/2024-04-30/2024-04-30/text/original/epub/OEBPS/document_1/document_1.html#_Toc166157837> ;
    dcat:landingPage "https://www.legislation.gov.au/F2021L00319/2024-04-30/2024-04-30/text/original/epub/OEBPS/document_1/document_1.html#_Toc166157837"^^xsd:anyURI ;
    dcat:theme legcons:Item .

F2021L00319:400 a legcons:Item,
        owl:Class,
        dcat:Resource ;
    rdfs:label "Item - I400 12 18  Notice requiring accredited veterinarian to undertake further training given before commencement time"@en-AU ;
    dct:isPartOf F2021L00319:397 ;
    dct:isReferencedBy F2021L00319: ;
    rdfs:comment "12 18  Notice requiring accredited veterinarian to undertake further training given before commencement time - Abrievated Graph Key: I400"@en-AU ;
    skos:definition "12 18  Notice requiring accredited veterinarian to undertake further training given before commencement time"@en-AU ;
    skos:narrower F2021L00319:397 ;
    skos:prefLabel "Item I400"@en-AU ;
    dcat:accessURL <https://www.legislation.gov.au/F2021L00319/2024-04-30/2024-04-30/text/original/epub/OEBPS/document_1/document_1.html#_Toc166158233> ;
    dcat:landingPage "https://www.legislation.gov.au/F2021L00319/2024-04-30/2024-04-30/text/original/epub/OEBPS/document_1/document_1.html#_Toc166158233"^^xsd:anyURI ;
    dcat:theme legcons:Item .

F2021L00319:401 a legcons:Item,
        owl:Class,
        dcat:Resource ;
    rdfs:label "Item - I401 12 19  Application to vary accreditation made but not decided before commencement time"@en-AU ;
    dct:isPartOf F2021L00319:397 ;
    dct:isReferencedBy F2021L00319: ;
    rdfs:comment "12 19  Application to vary accreditation made but not decided before commencement time - Abrievated Graph Key: I401"@en-AU ;
    skos:definition "12 19  Application to vary accreditation made but not decided before commencement time"@en-AU ;
    skos:narrower F2021L00319:397 ;
    skos:prefLabel "Item I401"@en-AU ;
    dcat:accessURL <https://www.legislation.gov.au/F2021L00319/2024-04-30/2024-04-30/text/original/epub/OEBPS/document_1/document_1.html#_Toc166158234> ;
    dcat:landingPage "https://www.legislation.gov.au/F2021L00319/2024-04-30/2024-04-30/text/original/epub/OEBPS/document_1/document_1.html#_Toc166158234"^^xsd:anyURI ;
    dcat:theme legcons:Item .

F2021L00319:402 a legcons:Item,
        owl:Class,
        dcat:Resource ;
    rdfs:label "Item - I402 12 20  Notice of varied conditions of accreditation given before commencement time to take effect after that time"@en-AU ;
    dct:isPartOf F2021L00319:397 ;
    dct:isReferencedBy F2021L00319: ;
    rdfs:comment "12 20  Notice of varied conditions of accreditation given before commencement time to take effect after that time - Abrievated Graph Key: I402"@en-AU ;
    skos:definition "12 20  Notice of varied conditions of accreditation given before commencement time to take effect after that time"@en-AU ;
    skos:narrower F2021L00319:397 ;
    skos:prefLabel "Item I402"@en-AU ;
    dcat:accessURL <https://www.legislation.gov.au/F2021L00319/2024-04-30/2024-04-30/text/original/epub/OEBPS/document_1/document_1.html#_Toc166158235> ;
    dcat:landingPage "https://www.legislation.gov.au/F2021L00319/2024-04-30/2024-04-30/text/original/epub/OEBPS/document_1/document_1.html#_Toc166158235"^^xsd:anyURI ;
    dcat:theme legcons:Item .

F2021L00319:403 a legcons:Item,
        owl:Class,
        dcat:Resource ;
    rdfs:label "Item - I403 12 21  Suspension of accreditation"@en-AU ;
    dct:isPartOf F2021L00319:397 ;
    dct:isReferencedBy F2021L00319: ;
    rdfs:comment "12 21  Suspension of accreditation - Abrievated Graph Key: I403"@en-AU ;
    skos:definition "12 21  Suspension of accreditation"@en-AU ;
    skos:narrower F2021L00319:397 ;
    skos:prefLabel "Item I403"@en-AU ;
    dcat:accessURL <https://www.legislation.gov.au/F2021L00319/2024-04-30/2024-04-30/text/original/epub/OEBPS/document_1/document_1.html#_Toc166158236> ;
    dcat:landingPage "https://www.legislation.gov.au/F2021L00319/2024-04-30/2024-04-30/text/original/epub/OEBPS/document_1/document_1.html#_Toc166158236"^^xsd:anyURI ;
    dcat:theme legcons:Item .

F2021L00319:404 a legcons:Item,
        owl:Class,
        dcat:Resource ;
    rdfs:label "Item - I404 12 22  Revocation of accreditation"@en-AU ;
    dct:isPartOf F2021L00319:397 ;
    dct:isReferencedBy F2021L00319: ;
    rdfs:comment "12 22  Revocation of accreditation - Abrievated Graph Key: I404"@en-AU ;
    skos:definition "12 22  Revocation of accreditation"@en-AU ;
    skos:narrower F2021L00319:397 ;
    skos:prefLabel "Item I404"@en-AU ;
    dcat:accessURL <https://www.legislation.gov.au/F2021L00319/2024-04-30/2024-04-30/text/original/epub/OEBPS/document_1/document_1.html#_Toc166158237> ;
    dcat:landingPage "https://www.legislation.gov.au/F2021L00319/2024-04-30/2024-04-30/text/original/epub/OEBPS/document_1/document_1.html#_Toc166158237"^^xsd:anyURI ;
    dcat:theme legcons:Item .

F2021L00319:407 a legcons:Item,
        owl:Class,
        dcat:Resource ;
    rdfs:label "Item - I407 12 23  Exporters approved export program in force immediately before commencement time"@en-AU ;
    dct:isPartOf F2021L00319:406 ;
    dct:isReferencedBy F2021L00319: ;
    rdfs:comment "12 23  Exporters approved export program in force immediately before commencement time - Abrievated Graph Key: I407"@en-AU ;
    skos:definition "12 23  Exporters approved export program in force immediately before commencement time"@en-AU ;
    skos:narrower F2021L00319:406 ;
    skos:prefLabel "Item I407"@en-AU ;
    dcat:accessURL <https://www.legislation.gov.au/F2021L00319/2024-04-30/2024-04-30/text/original/epub/OEBPS/document_1/document_1.html#_Toc166158240> ;
    dcat:landingPage "https://www.legislation.gov.au/F2021L00319/2024-04-30/2024-04-30/text/original/epub/OEBPS/document_1/document_1.html#_Toc166158240"^^xsd:anyURI ;
    dcat:theme legcons:Item .

F2021L00319:408 a legcons:Item,
        owl:Class,
        dcat:Resource ;
    rdfs:label "Item - I408 12 24  Application for approval of program of export operations made but not decided before commencement time"@en-AU ;
    dct:isPartOf F2021L00319:406 ;
    dct:isReferencedBy F2021L00319: ;
    rdfs:comment "12 24  Application for approval of program of export operations made but not decided before commencement time - Abrievated Graph Key: I408"@en-AU ;
    skos:definition "12 24  Application for approval of program of export operations made but not decided before commencement time"@en-AU ;
    skos:narrower F2021L00319:406 ;
    skos:prefLabel "Item I408"@en-AU ;
    dcat:accessURL <https://www.legislation.gov.au/F2021L00319/2024-04-30/2024-04-30/text/original/epub/OEBPS/document_1/document_1.html#_Toc166158241> ;
    dcat:landingPage "https://www.legislation.gov.au/F2021L00319/2024-04-30/2024-04-30/text/original/epub/OEBPS/document_1/document_1.html#_Toc166158241"^^xsd:anyURI ;
    dcat:theme legcons:Item .

F2021L00319:409 a legcons:Item,
        owl:Class,
        dcat:Resource ;
    rdfs:label "Item - I409 12 25  Variation of approved export program"@en-AU ;
    dct:isPartOf F2021L00319:406 ;
    dct:isReferencedBy F2021L00319: ;
    rdfs:comment "12 25  Variation of approved export program - Abrievated Graph Key: I409"@en-AU ;
    skos:definition "12 25  Variation of approved export program"@en-AU ;
    skos:narrower F2021L00319:406 ;
    skos:prefLabel "Item I409"@en-AU ;
    dcat:accessURL <https://www.legislation.gov.au/F2021L00319/2024-04-30/2024-04-30/text/original/epub/OEBPS/document_1/document_1.html#_Toc166158242> ;
    dcat:landingPage "https://www.legislation.gov.au/F2021L00319/2024-04-30/2024-04-30/text/original/epub/OEBPS/document_1/document_1.html#_Toc166158242"^^xsd:anyURI ;
    dcat:theme legcons:Item .

F2021L00319:41 a legcons:Item,
        owl:Class,
        dcat:Resource ;
    rdfs:label "Item - I41 2 23  Application of this Division"@en-AU ;
    dct:isPartOf F2021L00319:40 ;
    dct:isReferencedBy F2021L00319: ;
    rdfs:comment "2 23  Application of this Division - Abrievated Graph Key: I41"@en-AU ;
    skos:definition "2 23  Application of this Division"@en-AU ;
    skos:narrower F2021L00319:40 ;
    skos:prefLabel "Item I41"@en-AU ;
    dcat:accessURL <https://www.legislation.gov.au/F2021L00319/2024-04-30/2024-04-30/text/original/epub/OEBPS/document_1/document_1.html#_Toc166157874> ;
    dcat:landingPage "https://www.legislation.gov.au/F2021L00319/2024-04-30/2024-04-30/text/original/epub/OEBPS/document_1/document_1.html#_Toc166157874"^^xsd:anyURI ;
    dcat:theme legcons:Item .

F2021L00319:410 a legcons:Item,
        owl:Class,
        dcat:Resource ;
    rdfs:label "Item - I410 12 26  Approved export program suspended before commencement time"@en-AU ;
    dct:isPartOf F2021L00319:406 ;
    dct:isReferencedBy F2021L00319: ;
    rdfs:comment "12 26  Approved export program suspended before commencement time - Abrievated Graph Key: I410"@en-AU ;
    skos:definition "12 26  Approved export program suspended before commencement time"@en-AU ;
    skos:narrower F2021L00319:406 ;
    skos:prefLabel "Item I410"@en-AU ;
    dcat:accessURL <https://www.legislation.gov.au/F2021L00319/2024-04-30/2024-04-30/text/original/epub/OEBPS/document_1/document_1.html#_Toc166158243> ;
    dcat:landingPage "https://www.legislation.gov.au/F2021L00319/2024-04-30/2024-04-30/text/original/epub/OEBPS/document_1/document_1.html#_Toc166158243"^^xsd:anyURI ;
    dcat:theme legcons:Item .

F2021L00319:411 a legcons:Item,
        owl:Class,
        dcat:Resource ;
    rdfs:label "Item - I411 12 27  Request by holder of approved export program to cancel suspension"@en-AU ;
    dct:isPartOf F2021L00319:406 ;
    dct:isReferencedBy F2021L00319: ;
    rdfs:comment "12 27  Request by holder of approved export program to cancel suspension - Abrievated Graph Key: I411"@en-AU ;
    skos:definition "12 27  Request by holder of approved export program to cancel suspension"@en-AU ;
    skos:narrower F2021L00319:406 ;
    skos:prefLabel "Item I411"@en-AU ;
    dcat:accessURL <https://www.legislation.gov.au/F2021L00319/2024-04-30/2024-04-30/text/original/epub/OEBPS/document_1/document_1.html#_Toc166158244> ;
    dcat:landingPage "https://www.legislation.gov.au/F2021L00319/2024-04-30/2024-04-30/text/original/epub/OEBPS/document_1/document_1.html#_Toc166158244"^^xsd:anyURI ;
    dcat:theme legcons:Item .

F2021L00319:412 a legcons:Item,
        owl:Class,
        dcat:Resource ;
    rdfs:label "Item - I412 12 28  Request to suspend approved export program made but not decided before commencement time"@en-AU ;
    dct:isPartOf F2021L00319:406 ;
    dct:isReferencedBy F2021L00319: ;
    rdfs:comment "12 28  Request to suspend approved export program made but not decided before commencement time - Abrievated Graph Key: I412"@en-AU ;
    skos:definition "12 28  Request to suspend approved export program made but not decided before commencement time"@en-AU ;
    skos:narrower F2021L00319:406 ;
    skos:prefLabel "Item I412"@en-AU ;
    dcat:accessURL <https://www.legislation.gov.au/F2021L00319/2024-04-30/2024-04-30/text/original/epub/OEBPS/document_1/document_1.html#_Toc166158245> ;
    dcat:landingPage "https://www.legislation.gov.au/F2021L00319/2024-04-30/2024-04-30/text/original/epub/OEBPS/document_1/document_1.html#_Toc166158245"^^xsd:anyURI ;
    dcat:theme legcons:Item .

F2021L00319:413 a legcons:Item,
        owl:Class,
        dcat:Resource ;
    rdfs:label "Item - I413 12 29  Cancellation of approved export program"@en-AU ;
    dct:isPartOf F2021L00319:406 ;
    dct:isReferencedBy F2021L00319: ;
    rdfs:comment "12 29  Cancellation of approved export program - Abrievated Graph Key: I413"@en-AU ;
    skos:definition "12 29  Cancellation of approved export program"@en-AU ;
    skos:narrower F2021L00319:406 ;
    skos:prefLabel "Item I413"@en-AU ;
    dcat:accessURL <https://www.legislation.gov.au/F2021L00319/2024-04-30/2024-04-30/text/original/epub/OEBPS/document_1/document_1.html#_Toc166158246> ;
    dcat:landingPage "https://www.legislation.gov.au/F2021L00319/2024-04-30/2024-04-30/text/original/epub/OEBPS/document_1/document_1.html#_Toc166158246"^^xsd:anyURI ;
    dcat:theme legcons:Item .

F2021L00319:415 a legcons:Item,
        owl:Class,
        dcat:Resource ;
    rdfs:label "Item - I415 12 30  Secretarys approved export program in force immediately before commencement time"@en-AU ;
    dct:isPartOf F2021L00319:414 ;
    dct:isReferencedBy F2021L00319: ;
    rdfs:comment "12 30  Secretarys approved export program in force immediately before commencement time - Abrievated Graph Key: I415"@en-AU ;
    skos:definition "12 30  Secretarys approved export program in force immediately before commencement time"@en-AU ;
    skos:narrower F2021L00319:414 ;
    skos:prefLabel "Item I415"@en-AU ;
    dcat:accessURL <https://www.legislation.gov.au/F2021L00319/2024-04-30/2024-04-30/text/original/epub/OEBPS/document_1/document_1.html#_Toc166158248> ;
    dcat:landingPage "https://www.legislation.gov.au/F2021L00319/2024-04-30/2024-04-30/text/original/epub/OEBPS/document_1/document_1.html#_Toc166158248"^^xsd:anyURI ;
    dcat:theme legcons:Item .

F2021L00319:416 a legcons:Item,
        owl:Class,
        dcat:Resource ;
    rdfs:label "Item - I416 12 31  Variation of approved export program before commencement time to take effect after commencement time"@en-AU ;
    dct:isPartOf F2021L00319:414 ;
    dct:isReferencedBy F2021L00319: ;
    rdfs:comment "12 31  Variation of approved export program before commencement time to take effect after commencement time - Abrievated Graph Key: I416"@en-AU ;
    skos:definition "12 31  Variation of approved export program before commencement time to take effect after commencement time"@en-AU ;
    skos:narrower F2021L00319:414 ;
    skos:prefLabel "Item I416"@en-AU ;
    dcat:accessURL <https://www.legislation.gov.au/F2021L00319/2024-04-30/2024-04-30/text/original/epub/OEBPS/document_1/document_1.html#_Toc166158249> ;
    dcat:landingPage "https://www.legislation.gov.au/F2021L00319/2024-04-30/2024-04-30/text/original/epub/OEBPS/document_1/document_1.html#_Toc166158249"^^xsd:anyURI ;
    dcat:theme legcons:Item .

F2021L00319:418 a legcons:Item,
        owl:Class,
        dcat:Resource ;
    rdfs:label "Item - I418 12 32  Application of amendments"@en-AU ;
    dct:isPartOf F2021L00319:417 ;
    dct:isReferencedBy F2021L00319: ;
    rdfs:comment "12 32  Application of amendments - Abrievated Graph Key: I418"@en-AU ;
    skos:definition "12 32  Application of amendments"@en-AU ;
    skos:narrower F2021L00319:417 ;
    skos:prefLabel "Item I418"@en-AU ;
    dcat:accessURL <https://www.legislation.gov.au/F2021L00319/2024-04-30/2024-04-30/text/original/epub/OEBPS/document_1/document_1.html#_Toc166158251> ;
    dcat:landingPage "https://www.legislation.gov.au/F2021L00319/2024-04-30/2024-04-30/text/original/epub/OEBPS/document_1/document_1.html#_Toc166158251"^^xsd:anyURI ;
    dcat:theme legcons:Item .

F2021L00319:42 a legcons:Item,
        owl:Class,
        dcat:Resource ;
    rdfs:label "Item - I42 2 24  Issuing body must consider conditions if any of approval of notice of intention to export consignment"@en-AU ;
    dct:isPartOf F2021L00319:40 ;
    dct:isReferencedBy F2021L00319: ;
    rdfs:comment "2 24  Issuing body must consider conditions if any of approval of notice of intention to export consignment - Abrievated Graph Key: I42"@en-AU ;
    skos:definition "2 24  Issuing body must consider conditions if any of approval of notice of intention to export consignment"@en-AU ;
    skos:narrower F2021L00319:40 ;
    skos:prefLabel "Item I42"@en-AU ;
    dcat:accessURL <https://www.legislation.gov.au/F2021L00319/2024-04-30/2024-04-30/text/original/epub/OEBPS/document_1/document_1.html#_Toc166157875> ;
    dcat:landingPage "https://www.legislation.gov.au/F2021L00319/2024-04-30/2024-04-30/text/original/epub/OEBPS/document_1/document_1.html#_Toc166157875"^^xsd:anyURI ;
    dcat:theme legcons:Item .

F2021L00319:420 a legcons:Item,
        owl:Class,
        dcat:Resource ;
    rdfs:label "Item - I420 12 33  Application of amendments"@en-AU ;
    dct:isPartOf F2021L00319:419 ;
    dct:isReferencedBy F2021L00319: ;
    rdfs:comment "12 33  Application of amendments - Abrievated Graph Key: I420"@en-AU ;
    skos:definition "12 33  Application of amendments"@en-AU ;
    skos:narrower F2021L00319:419 ;
    skos:prefLabel "Item I420"@en-AU ;
    dcat:accessURL <https://www.legislation.gov.au/F2021L00319/2024-04-30/2024-04-30/text/original/epub/OEBPS/document_1/document_1.html#_Toc166158253> ;
    dcat:landingPage "https://www.legislation.gov.au/F2021L00319/2024-04-30/2024-04-30/text/original/epub/OEBPS/document_1/document_1.html#_Toc166158253"^^xsd:anyURI ;
    dcat:theme legcons:Item .

F2021L00319:422 a legcons:Item,
        owl:Class,
        dcat:Resource ;
    rdfs:label "Item - I422 12 34  Definitions"@en-AU ;
    dct:isPartOf F2021L00319:421 ;
    dct:isReferencedBy F2021L00319: ;
    rdfs:comment "12 34  Definitions - Abrievated Graph Key: I422"@en-AU ;
    skos:definition "12 34  Definitions"@en-AU ;
    skos:narrower F2021L00319:421 ;
    skos:prefLabel "Item I422"@en-AU ;
    dcat:accessURL <https://www.legislation.gov.au/F2021L00319/2024-04-30/2024-04-30/text/original/epub/OEBPS/document_1/document_1.html#_Toc166158255> ;
    dcat:landingPage "https://www.legislation.gov.au/F2021L00319/2024-04-30/2024-04-30/text/original/epub/OEBPS/document_1/document_1.html#_Toc166158255"^^xsd:anyURI ;
    dcat:theme legcons:Item .

F2021L00319:423 a legcons:Item,
        owl:Class,
        dcat:Resource ;
    rdfs:label "Item - I423 12 35  Conditions of approved arrangements"@en-AU ;
    dct:isPartOf F2021L00319:421 ;
    dct:isReferencedBy F2021L00319: ;
    rdfs:comment "12 35  Conditions of approved arrangements - Abrievated Graph Key: I423"@en-AU ;
    skos:definition "12 35  Conditions of approved arrangements"@en-AU ;
    skos:narrower F2021L00319:421 ;
    skos:prefLabel "Item I423"@en-AU ;
    dcat:accessURL <https://www.legislation.gov.au/F2021L00319/2024-04-30/2024-04-30/text/original/epub/OEBPS/document_1/document_1.html#_Toc166158256> ;
    dcat:landingPage "https://www.legislation.gov.au/F2021L00319/2024-04-30/2024-04-30/text/original/epub/OEBPS/document_1/document_1.html#_Toc166158256"^^xsd:anyURI ;
    dcat:theme legcons:Item .

F2021L00319:424 a legcons:Item,
        owl:Class,
        dcat:Resource ;
    rdfs:label "Item - I424 12 36  Conditions of livestock export licenceorders made by authorised officers"@en-AU ;
    dct:isPartOf F2021L00319:421 ;
    dct:isReferencedBy F2021L00319: ;
    rdfs:comment "12 36  Conditions of livestock export licenceorders made by authorised officers - Abrievated Graph Key: I424"@en-AU ;
    skos:definition "12 36  Conditions of livestock export licenceorders made by authorised officers"@en-AU ;
    skos:narrower F2021L00319:421 ;
    skos:prefLabel "Item I424"@en-AU ;
    dcat:accessURL <https://www.legislation.gov.au/F2021L00319/2024-04-30/2024-04-30/text/original/epub/OEBPS/document_1/document_1.html#_Toc166158257> ;
    dcat:landingPage "https://www.legislation.gov.au/F2021L00319/2024-04-30/2024-04-30/text/original/epub/OEBPS/document_1/document_1.html#_Toc166158257"^^xsd:anyURI ;
    dcat:theme legcons:Item .

F2021L00319:425 a legcons:Item,
        owl:Class,
        dcat:Resource ;
    rdfs:label "Item - I425 12 37  Revocation of approved ESCAS"@en-AU ;
    dct:isPartOf F2021L00319:421 ;
    dct:isReferencedBy F2021L00319: ;
    rdfs:comment "12 37  Revocation of approved ESCAS - Abrievated Graph Key: I425"@en-AU ;
    skos:definition "12 37  Revocation of approved ESCAS"@en-AU ;
    skos:narrower F2021L00319:421 ;
    skos:prefLabel "Item I425"@en-AU ;
    dcat:accessURL <https://www.legislation.gov.au/F2021L00319/2024-04-30/2024-04-30/text/original/epub/OEBPS/document_1/document_1.html#_Toc166158258> ;
    dcat:landingPage "https://www.legislation.gov.au/F2021L00319/2024-04-30/2024-04-30/text/original/epub/OEBPS/document_1/document_1.html#_Toc166158258"^^xsd:anyURI ;
    dcat:theme legcons:Item .

F2021L00319:426 a legcons:Item,
        owl:Class,
        dcat:Resource ;
    rdfs:label "Item - I426 12 38  Revocation of approval of notice of intention to export consignment"@en-AU ;
    dct:isPartOf F2021L00319:421 ;
    dct:isReferencedBy F2021L00319: ;
    rdfs:comment "12 38  Revocation of approval of notice of intention to export consignment - Abrievated Graph Key: I426"@en-AU ;
    skos:definition "12 38  Revocation of approval of notice of intention to export consignment"@en-AU ;
    skos:narrower F2021L00319:421 ;
    skos:prefLabel "Item I426"@en-AU ;
    dcat:accessURL <https://www.legislation.gov.au/F2021L00319/2024-04-30/2024-04-30/text/original/epub/OEBPS/document_1/document_1.html#_Toc166158259> ;
    dcat:landingPage "https://www.legislation.gov.au/F2021L00319/2024-04-30/2024-04-30/text/original/epub/OEBPS/document_1/document_1.html#_Toc166158259"^^xsd:anyURI ;
    dcat:theme legcons:Item .

F2021L00319:428 a legcons:Item,
        owl:Class,
        dcat:Resource ;
    rdfs:label "Item - I428 Endnote 1 About the endnotes"@en-AU ;
    dct:isPartOf F2021L00319:427 ;
    dct:isReferencedBy F2021L00319: ;
    rdfs:comment "Endnote 1 About the endnotes - Abrievated Graph Key: I428"@en-AU ;
    skos:definition "Endnote 1 About the endnotes"@en-AU ;
    skos:narrower F2021L00319:427 ;
    skos:prefLabel "Item I428"@en-AU ;
    dcat:accessURL <https://www.legislation.gov.au/F2021L00319/2024-04-30/2024-04-30/text/original/epub/OEBPS/document_1/document_1.html#_Toc166158261> ;
    dcat:landingPage "https://www.legislation.gov.au/F2021L00319/2024-04-30/2024-04-30/text/original/epub/OEBPS/document_1/document_1.html#_Toc166158261"^^xsd:anyURI ;
    dcat:theme legcons:Item .

F2021L00319:429 a legcons:Item,
        owl:Class,
        dcat:Resource ;
    rdfs:label "Item - I429 Endnote 2 Abbreviation key"@en-AU ;
    dct:isPartOf F2021L00319:427 ;
    dct:isReferencedBy F2021L00319: ;
    rdfs:comment "Endnote 2 Abbreviation key - Abrievated Graph Key: I429"@en-AU ;
    skos:definition "Endnote 2 Abbreviation key"@en-AU ;
    skos:narrower F2021L00319:427 ;
    skos:prefLabel "Item I429"@en-AU ;
    dcat:accessURL <https://www.legislation.gov.au/F2021L00319/2024-04-30/2024-04-30/text/original/epub/OEBPS/document_1/document_1.html#_Toc166158262> ;
    dcat:landingPage "https://www.legislation.gov.au/F2021L00319/2024-04-30/2024-04-30/text/original/epub/OEBPS/document_1/document_1.html#_Toc166158262"^^xsd:anyURI ;
    dcat:theme legcons:Item .

F2021L00319:430 a legcons:Item,
        owl:Class,
        dcat:Resource ;
    rdfs:label "Item - I430 Endnote 3 Legislation history"@en-AU ;
    dct:isPartOf F2021L00319:427 ;
    dct:isReferencedBy F2021L00319: ;
    rdfs:comment "Endnote 3 Legislation history - Abrievated Graph Key: I430"@en-AU ;
    skos:definition "Endnote 3 Legislation history"@en-AU ;
    skos:narrower F2021L00319:427 ;
    skos:prefLabel "Item I430"@en-AU ;
    dcat:accessURL <https://www.legislation.gov.au/F2021L00319/2024-04-30/2024-04-30/text/original/epub/OEBPS/document_1/document_1.html#_Toc166158263> ;
    dcat:landingPage "https://www.legislation.gov.au/F2021L00319/2024-04-30/2024-04-30/text/original/epub/OEBPS/document_1/document_1.html#_Toc166158263"^^xsd:anyURI ;
    dcat:theme legcons:Item .

F2021L00319:431 a legcons:Item,
        owl:Class,
        dcat:Resource ;
    rdfs:label "Item - I431 Endnote 4 Amendment history"@en-AU ;
    dct:isPartOf F2021L00319:427 ;
    dct:isReferencedBy F2021L00319: ;
    rdfs:comment "Endnote 4 Amendment history - Abrievated Graph Key: I431"@en-AU ;
    skos:definition "Endnote 4 Amendment history"@en-AU ;
    skos:narrower F2021L00319:427 ;
    skos:prefLabel "Item I431"@en-AU ;
    dcat:accessURL <https://www.legislation.gov.au/F2021L00319/2024-04-30/2024-04-30/text/original/epub/OEBPS/document_1/document_1.html#_Toc166158264> ;
    dcat:landingPage "https://www.legislation.gov.au/F2021L00319/2024-04-30/2024-04-30/text/original/epub/OEBPS/document_1/document_1.html#_Toc166158264"^^xsd:anyURI ;
    dcat:theme legcons:Item .

F2021L00319:45 a legcons:Item,
        owl:Class,
        dcat:Resource ;
    rdfs:label "Item - I45 4 1  Application of this Chapter"@en-AU ;
    dct:isPartOf F2021L00319:44 ;
    dct:isReferencedBy F2021L00319: ;
    rdfs:comment "4 1  Application of this Chapter - Abrievated Graph Key: I45"@en-AU ;
    skos:definition "4 1  Application of this Chapter"@en-AU ;
    skos:narrower F2021L00319:44 ;
    skos:prefLabel "Item I45"@en-AU ;
    dcat:accessURL <https://www.legislation.gov.au/F2021L00319/2024-04-30/2024-04-30/text/original/epub/OEBPS/document_1/document_1.html#_Toc166157878> ;
    dcat:landingPage "https://www.legislation.gov.au/F2021L00319/2024-04-30/2024-04-30/text/original/epub/OEBPS/document_1/document_1.html#_Toc166157878"^^xsd:anyURI ;
    dcat:theme legcons:Item .

F2021L00319:48 a legcons:Item,
        owl:Class,
        dcat:Resource ;
    rdfs:label "Item - I48 4 2  Matters relating to construction equipment and facilities"@en-AU ;
    dct:isPartOf F2021L00319:47 ;
    dct:isReferencedBy F2021L00319: ;
    rdfs:comment "4 2  Matters relating to construction equipment and facilities - Abrievated Graph Key: I48"@en-AU ;
    skos:definition "4 2  Matters relating to construction equipment and facilities"@en-AU ;
    skos:narrower F2021L00319:47 ;
    skos:prefLabel "Item I48"@en-AU ;
    dcat:accessURL <https://www.legislation.gov.au/F2021L00319/2024-04-30/2024-04-30/text/original/epub/OEBPS/document_1/document_1.html#_Toc166157881> ;
    dcat:landingPage "https://www.legislation.gov.au/F2021L00319/2024-04-30/2024-04-30/text/original/epub/OEBPS/document_1/document_1.html#_Toc166157881"^^xsd:anyURI ;
    dcat:theme legcons:Item .

F2021L00319:49 a legcons:Item,
        owl:Class,
        dcat:Resource ;
    rdfs:label "Item - I49 4 3  Other requirements for registration"@en-AU ;
    dct:isPartOf F2021L00319:47 ;
    dct:isReferencedBy F2021L00319: ;
    rdfs:comment "4 3  Other requirements for registration - Abrievated Graph Key: I49"@en-AU ;
    skos:definition "4 3  Other requirements for registration"@en-AU ;
    skos:narrower F2021L00319:47 ;
    skos:prefLabel "Item I49"@en-AU ;
    dcat:accessURL <https://www.legislation.gov.au/F2021L00319/2024-04-30/2024-04-30/text/original/epub/OEBPS/document_1/document_1.html#_Toc166157882> ;
    dcat:landingPage "https://www.legislation.gov.au/F2021L00319/2024-04-30/2024-04-30/text/original/epub/OEBPS/document_1/document_1.html#_Toc166157882"^^xsd:anyURI ;
    dcat:theme legcons:Item .

F2021L00319:5 a legcons:Item,
        owl:Class,
        dcat:Resource ;
    rdfs:label "Item - I5 1 4  Application of this instrument"@en-AU ;
    dct:isPartOf F2021L00319:1 ;
    dct:isReferencedBy F2021L00319: ;
    rdfs:comment "1 4  Application of this instrument - Abrievated Graph Key: I5"@en-AU ;
    skos:definition "1 4  Application of this instrument"@en-AU ;
    skos:narrower F2021L00319:1 ;
    skos:prefLabel "Item I5"@en-AU ;
    dcat:accessURL <https://www.legislation.gov.au/F2021L00319/2024-04-30/2024-04-30/text/original/epub/OEBPS/document_1/document_1.html#_Toc166157838> ;
    dcat:landingPage "https://www.legislation.gov.au/F2021L00319/2024-04-30/2024-04-30/text/original/epub/OEBPS/document_1/document_1.html#_Toc166157838"^^xsd:anyURI ;
    dcat:theme legcons:Item .

F2021L00319:51 a legcons:Item,
        owl:Class,
        dcat:Resource ;
    rdfs:label "Item - I51 4 4  Period of effect of registration"@en-AU ;
    dct:isPartOf F2021L00319:50 ;
    dct:isReferencedBy F2021L00319: ;
    rdfs:comment "4 4  Period of effect of registration - Abrievated Graph Key: I51"@en-AU ;
    skos:definition "4 4  Period of effect of registration"@en-AU ;
    skos:narrower F2021L00319:50 ;
    skos:prefLabel "Item I51"@en-AU ;
    dcat:accessURL <https://www.legislation.gov.au/F2021L00319/2024-04-30/2024-04-30/text/original/epub/OEBPS/document_1/document_1.html#_Toc166157884> ;
    dcat:landingPage "https://www.legislation.gov.au/F2021L00319/2024-04-30/2024-04-30/text/original/epub/OEBPS/document_1/document_1.html#_Toc166157884"^^xsd:anyURI ;
    dcat:theme legcons:Item .

F2021L00319:53 a legcons:Item,
        owl:Class,
        dcat:Resource ;
    rdfs:label "Item - I53 4 5  Purpose of this Part"@en-AU ;
    dct:isPartOf F2021L00319:52 ;
    dct:isReferencedBy F2021L00319: ;
    rdfs:comment "4 5  Purpose of this Part - Abrievated Graph Key: I53"@en-AU ;
    skos:definition "4 5  Purpose of this Part"@en-AU ;
    skos:narrower F2021L00319:52 ;
    skos:prefLabel "Item I53"@en-AU ;
    dcat:accessURL <https://www.legislation.gov.au/F2021L00319/2024-04-30/2024-04-30/text/original/epub/OEBPS/document_1/document_1.html#_Toc166157886> ;
    dcat:landingPage "https://www.legislation.gov.au/F2021L00319/2024-04-30/2024-04-30/text/original/epub/OEBPS/document_1/document_1.html#_Toc166157886"^^xsd:anyURI ;
    dcat:theme legcons:Item .

F2021L00319:54 a legcons:Item,
        owl:Class,
        dcat:Resource ;
    rdfs:label "Item - I54 4 5 A  Australian Standards for the Export of Livestock"@en-AU ;
    dct:isPartOf F2021L00319:52 ;
    dct:isReferencedBy F2021L00319: ;
    rdfs:comment "4 5 A  Australian Standards for the Export of Livestock - Abrievated Graph Key: I54"@en-AU ;
    skos:definition "4 5 A  Australian Standards for the Export of Livestock"@en-AU ;
    skos:narrower F2021L00319:52 ;
    skos:prefLabel "Item I54"@en-AU ;
    dcat:accessURL <https://www.legislation.gov.au/F2021L00319/2024-04-30/2024-04-30/text/original/epub/OEBPS/document_1/document_1.html#_Toc166157887> ;
    dcat:landingPage "https://www.legislation.gov.au/F2021L00319/2024-04-30/2024-04-30/text/original/epub/OEBPS/document_1/document_1.html#_Toc166157887"^^xsd:anyURI ;
    dcat:theme legcons:Item .

F2021L00319:55 a legcons:Item,
        owl:Class,
        dcat:Resource ;
    rdfs:label "Item - I55 4 6  Prescribed livestock at establishment must be covered by registration and approved arrangement or operations and governance manual"@en-AU ;
    dct:isPartOf F2021L00319:52 ;
    dct:isReferencedBy F2021L00319: ;
    rdfs:comment "4 6  Prescribed livestock at establishment must be covered by registration and approved arrangement or operations and governance manual - Abrievated Graph Key: I55"@en-AU ;
    skos:definition "4 6  Prescribed livestock at establishment must be covered by registration and approved arrangement or operations and governance manual"@en-AU ;
    skos:narrower F2021L00319:52 ;
    skos:prefLabel "Item I55"@en-AU ;
    dcat:accessURL <https://www.legislation.gov.au/F2021L00319/2024-04-30/2024-04-30/text/original/epub/OEBPS/document_1/document_1.html#_Toc166157888> ;
    dcat:landingPage "https://www.legislation.gov.au/F2021L00319/2024-04-30/2024-04-30/text/original/epub/OEBPS/document_1/document_1.html#_Toc166157888"^^xsd:anyURI ;
    dcat:theme legcons:Item .

F2021L00319:56 a legcons:Item,
        owl:Class,
        dcat:Resource ;
    rdfs:label "Item - I56 4 7  Occupier must provide reasonable assistance to accredited veterinarian"@en-AU ;
    dct:isPartOf F2021L00319:52 ;
    dct:isReferencedBy F2021L00319: ;
    rdfs:comment "4 7  Occupier must provide reasonable assistance to accredited veterinarian - Abrievated Graph Key: I56"@en-AU ;
    skos:definition "4 7  Occupier must provide reasonable assistance to accredited veterinarian"@en-AU ;
    skos:narrower F2021L00319:52 ;
    skos:prefLabel "Item I56"@en-AU ;
    dcat:accessURL <https://www.legislation.gov.au/F2021L00319/2024-04-30/2024-04-30/text/original/epub/OEBPS/document_1/document_1.html#_Toc166157889> ;
    dcat:landingPage "https://www.legislation.gov.au/F2021L00319/2024-04-30/2024-04-30/text/original/epub/OEBPS/document_1/document_1.html#_Toc166157889"^^xsd:anyURI ;
    dcat:theme legcons:Item .

F2021L00319:57 a legcons:Item,
        owl:Class,
        dcat:Resource ;
    rdfs:label "Item - I57 4 8  Compliance with operations manual"@en-AU ;
    dct:isPartOf F2021L00319:52 ;
    dct:isReferencedBy F2021L00319: ;
    rdfs:comment "4 8  Compliance with operations manual - Abrievated Graph Key: I57"@en-AU ;
    skos:definition "4 8  Compliance with operations manual"@en-AU ;
    skos:narrower F2021L00319:52 ;
    skos:prefLabel "Item I57"@en-AU ;
    dcat:accessURL <https://www.legislation.gov.au/F2021L00319/2024-04-30/2024-04-30/text/original/epub/OEBPS/document_1/document_1.html#_Toc166157890> ;
    dcat:landingPage "https://www.legislation.gov.au/F2021L00319/2024-04-30/2024-04-30/text/original/epub/OEBPS/document_1/document_1.html#_Toc166157890"^^xsd:anyURI ;
    dcat:theme legcons:Item .

F2021L00319:58 a legcons:Item,
        owl:Class,
        dcat:Resource ;
    rdfs:label "Item - I58 4 9  Variation of operations manual"@en-AU ;
    dct:isPartOf F2021L00319:52 ;
    dct:isReferencedBy F2021L00319: ;
    rdfs:comment "4 9  Variation of operations manual - Abrievated Graph Key: I58"@en-AU ;
    skos:definition "4 9  Variation of operations manual"@en-AU ;
    skos:narrower F2021L00319:52 ;
    skos:prefLabel "Item I58"@en-AU ;
    dcat:accessURL <https://www.legislation.gov.au/F2021L00319/2024-04-30/2024-04-30/text/original/epub/OEBPS/document_1/document_1.html#_Toc166157891> ;
    dcat:landingPage "https://www.legislation.gov.au/F2021L00319/2024-04-30/2024-04-30/text/original/epub/OEBPS/document_1/document_1.html#_Toc166157891"^^xsd:anyURI ;
    dcat:theme legcons:Item .

F2021L00319:6 a legcons:Item,
        owl:Class,
        dcat:Resource ;
    rdfs:label "Item - I6 1 5  Simplified outline of this instrument"@en-AU ;
    dct:isPartOf F2021L00319:1 ;
    dct:isReferencedBy F2021L00319: ;
    rdfs:comment "1 5  Simplified outline of this instrument - Abrievated Graph Key: I6"@en-AU ;
    skos:definition "1 5  Simplified outline of this instrument"@en-AU ;
    skos:narrower F2021L00319:1 ;
    skos:prefLabel "Item I6"@en-AU ;
    dcat:accessURL <https://www.legislation.gov.au/F2021L00319/2024-04-30/2024-04-30/text/original/epub/OEBPS/document_1/document_1.html#_Toc166157839> ;
    dcat:landingPage "https://www.legislation.gov.au/F2021L00319/2024-04-30/2024-04-30/text/original/epub/OEBPS/document_1/document_1.html#_Toc166157839"^^xsd:anyURI ;
    dcat:theme legcons:Item .

F2021L00319:60 a legcons:Item,
        owl:Class,
        dcat:Resource ;
    rdfs:label "Item - I60 4 10  Period within which application to renew registration must be made"@en-AU ;
    dct:isPartOf F2021L00319:59 ;
    dct:isReferencedBy F2021L00319: ;
    rdfs:comment "4 10  Period within which application to renew registration must be made - Abrievated Graph Key: I60"@en-AU ;
    skos:definition "4 10  Period within which application to renew registration must be made"@en-AU ;
    skos:narrower F2021L00319:59 ;
    skos:prefLabel "Item I60"@en-AU ;
    dcat:accessURL <https://www.legislation.gov.au/F2021L00319/2024-04-30/2024-04-30/text/original/epub/OEBPS/document_1/document_1.html#_Toc166157893> ;
    dcat:landingPage "https://www.legislation.gov.au/F2021L00319/2024-04-30/2024-04-30/text/original/epub/OEBPS/document_1/document_1.html#_Toc166157893"^^xsd:anyURI ;
    dcat:theme legcons:Item .

F2021L00319:61 a legcons:Item,
        owl:Class,
        dcat:Resource ;
    rdfs:label "Item - I61 4 11  Requirements for renewal of registration"@en-AU ;
    dct:isPartOf F2021L00319:59 ;
    dct:isReferencedBy F2021L00319: ;
    rdfs:comment "4 11  Requirements for renewal of registration - Abrievated Graph Key: I61"@en-AU ;
    skos:definition "4 11  Requirements for renewal of registration"@en-AU ;
    skos:narrower F2021L00319:59 ;
    skos:prefLabel "Item I61"@en-AU ;
    dcat:accessURL <https://www.legislation.gov.au/F2021L00319/2024-04-30/2024-04-30/text/original/epub/OEBPS/document_1/document_1.html#_Toc166157894> ;
    dcat:landingPage "https://www.legislation.gov.au/F2021L00319/2024-04-30/2024-04-30/text/original/epub/OEBPS/document_1/document_1.html#_Toc166157894"^^xsd:anyURI ;
    dcat:theme legcons:Item .

F2021L00319:63 a legcons:Item,
        owl:Class,
        dcat:Resource ;
    rdfs:label "Item - I63 4 12  Variation by Secretaryother reasons for varying registration"@en-AU ;
    dct:isPartOf F2021L00319:62 ;
    dct:isReferencedBy F2021L00319: ;
    rdfs:comment "4 12  Variation by Secretaryother reasons for varying registration - Abrievated Graph Key: I63"@en-AU ;
    skos:definition "4 12  Variation by Secretaryother reasons for varying registration"@en-AU ;
    skos:narrower F2021L00319:62 ;
    skos:prefLabel "Item I63"@en-AU ;
    dcat:accessURL <https://www.legislation.gov.au/F2021L00319/2024-04-30/2024-04-30/text/original/epub/OEBPS/document_1/document_1.html#_Toc166157896> ;
    dcat:landingPage "https://www.legislation.gov.au/F2021L00319/2024-04-30/2024-04-30/text/original/epub/OEBPS/document_1/document_1.html#_Toc166157896"^^xsd:anyURI ;
    dcat:theme legcons:Item .

F2021L00319:65 a legcons:Item,
        owl:Class,
        dcat:Resource ;
    rdfs:label "Item - I65 4 13  Other grounds for suspension"@en-AU ;
    dct:isPartOf F2021L00319:64 ;
    dct:isReferencedBy F2021L00319: ;
    rdfs:comment "4 13  Other grounds for suspension - Abrievated Graph Key: I65"@en-AU ;
    skos:definition "4 13  Other grounds for suspension"@en-AU ;
    skos:narrower F2021L00319:64 ;
    skos:prefLabel "Item I65"@en-AU ;
    dcat:accessURL <https://www.legislation.gov.au/F2021L00319/2024-04-30/2024-04-30/text/original/epub/OEBPS/document_1/document_1.html#_Toc166157898> ;
    dcat:landingPage "https://www.legislation.gov.au/F2021L00319/2024-04-30/2024-04-30/text/original/epub/OEBPS/document_1/document_1.html#_Toc166157898"^^xsd:anyURI ;
    dcat:theme legcons:Item .

F2021L00319:67 a legcons:Item,
        owl:Class,
        dcat:Resource ;
    rdfs:label "Item - I67 4 14  Other grounds for revocation"@en-AU ;
    dct:isPartOf F2021L00319:66 ;
    dct:isReferencedBy F2021L00319: ;
    rdfs:comment "4 14  Other grounds for revocation - Abrievated Graph Key: I67"@en-AU ;
    skos:definition "4 14  Other grounds for revocation"@en-AU ;
    skos:narrower F2021L00319:66 ;
    skos:prefLabel "Item I67"@en-AU ;
    dcat:accessURL <https://www.legislation.gov.au/F2021L00319/2024-04-30/2024-04-30/text/original/epub/OEBPS/document_1/document_1.html#_Toc166157900> ;
    dcat:landingPage "https://www.legislation.gov.au/F2021L00319/2024-04-30/2024-04-30/text/original/epub/OEBPS/document_1/document_1.html#_Toc166157900"^^xsd:anyURI ;
    dcat:theme legcons:Item .

F2021L00319:69 a legcons:Item,
        owl:Class,
        dcat:Resource ;
    rdfs:label "Item - I69 4 15  Application of this Part"@en-AU ;
    dct:isPartOf F2021L00319:68 ;
    dct:isReferencedBy F2021L00319: ;
    rdfs:comment "4 15  Application of this Part - Abrievated Graph Key: I69"@en-AU ;
    skos:definition "4 15  Application of this Part"@en-AU ;
    skos:narrower F2021L00319:68 ;
    skos:prefLabel "Item I69"@en-AU ;
    dcat:accessURL <https://www.legislation.gov.au/F2021L00319/2024-04-30/2024-04-30/text/original/epub/OEBPS/document_1/document_1.html#_Toc166157902> ;
    dcat:landingPage "https://www.legislation.gov.au/F2021L00319/2024-04-30/2024-04-30/text/original/epub/OEBPS/document_1/document_1.html#_Toc166157902"^^xsd:anyURI ;
    dcat:theme legcons:Item .

F2021L00319:7 a legcons:Part,
        owl:Class,
        dcat:Resource ;
    rdfs:label "Part - P7 Part 2 Interpretation"@en-AU ;
    dct:isPartOf F2021L00319:1 ;
    dct:isReferencedBy F2021L00319: ;
    rdfs:comment "Part 2 Interpretation - Abrievated Graph Key: P7"@en-AU ;
    skos:definition "Part 2 Interpretation"@en-AU ;
    skos:narrower F2021L00319:1 ;
    skos:prefLabel "Part P7"@en-AU ;
    dcat:accessURL <https://www.legislation.gov.au/F2021L00319/2024-04-30/2024-04-30/text/original/epub/OEBPS/document_1/document_1.html#_Toc166157840> ;
    dcat:landingPage "https://www.legislation.gov.au/F2021L00319/2024-04-30/2024-04-30/text/original/epub/OEBPS/document_1/document_1.html#_Toc166157840"^^xsd:anyURI ;
    dcat:theme legcons:Part .

F2021L00319:70 a legcons:Item,
        owl:Class,
        dcat:Resource ;
    rdfs:label "Item - I70 4 16  Initial consideration period"@en-AU ;
    dct:isPartOf F2021L00319:68 ;
    dct:isReferencedBy F2021L00319: ;
    rdfs:comment "4 16  Initial consideration period - Abrievated Graph Key: I70"@en-AU ;
    skos:definition "4 16  Initial consideration period"@en-AU ;
    skos:narrower F2021L00319:68 ;
    skos:prefLabel "Item I70"@en-AU ;
    dcat:accessURL <https://www.legislation.gov.au/F2021L00319/2024-04-30/2024-04-30/text/original/epub/OEBPS/document_1/document_1.html#_Toc166157903> ;
    dcat:landingPage "https://www.legislation.gov.au/F2021L00319/2024-04-30/2024-04-30/text/original/epub/OEBPS/document_1/document_1.html#_Toc166157903"^^xsd:anyURI ;
    dcat:theme legcons:Item .

F2021L00319:71 a legcons:Item,
        owl:Class,
        dcat:Resource ;
    rdfs:label "Item - I71 4 17  Maximum period within which request relating to application must be complied with"@en-AU ;
    dct:isPartOf F2021L00319:68 ;
    dct:isReferencedBy F2021L00319: ;
    rdfs:comment "4 17  Maximum period within which request relating to application must be complied with - Abrievated Graph Key: I71"@en-AU ;
    skos:definition "4 17  Maximum period within which request relating to application must be complied with"@en-AU ;
    skos:narrower F2021L00319:68 ;
    skos:prefLabel "Item I71"@en-AU ;
    dcat:accessURL <https://www.legislation.gov.au/F2021L00319/2024-04-30/2024-04-30/text/original/epub/OEBPS/document_1/document_1.html#_Toc166157904> ;
    dcat:landingPage "https://www.legislation.gov.au/F2021L00319/2024-04-30/2024-04-30/text/original/epub/OEBPS/document_1/document_1.html#_Toc166157904"^^xsd:anyURI ;
    dcat:theme legcons:Item .

F2021L00319:73 a legcons:Item,
        owl:Class,
        dcat:Resource ;
    rdfs:label "Item - I73 4 18  Secretary may publish information in reports relating to prescribed livestock"@en-AU ;
    dct:isPartOf F2021L00319:72 ;
    dct:isReferencedBy F2021L00319: ;
    rdfs:comment "4 18  Secretary may publish information in reports relating to prescribed livestock - Abrievated Graph Key: I73"@en-AU ;
    skos:definition "4 18  Secretary may publish information in reports relating to prescribed livestock"@en-AU ;
    skos:narrower F2021L00319:72 ;
    skos:prefLabel "Item I73"@en-AU ;
    dcat:accessURL <https://www.legislation.gov.au/F2021L00319/2024-04-30/2024-04-30/text/original/epub/OEBPS/document_1/document_1.html#_Toc166157906> ;
    dcat:landingPage "https://www.legislation.gov.au/F2021L00319/2024-04-30/2024-04-30/text/original/epub/OEBPS/document_1/document_1.html#_Toc166157906"^^xsd:anyURI ;
    dcat:theme legcons:Item .

F2021L00319:77 a legcons:Item,
        owl:Class,
        dcat:Resource ;
    rdfs:label "Item - I77 5 1  Other requirements for approval"@en-AU ;
    dct:isPartOf F2021L00319:76 ;
    dct:isReferencedBy F2021L00319: ;
    rdfs:comment "5 1  Other requirements for approval - Abrievated Graph Key: I77"@en-AU ;
    skos:definition "5 1  Other requirements for approval"@en-AU ;
    skos:narrower F2021L00319:76 ;
    skos:prefLabel "Item I77"@en-AU ;
    dcat:accessURL <https://www.legislation.gov.au/F2021L00319/2024-04-30/2024-04-30/text/original/epub/OEBPS/document_1/document_1.html#_Toc166157910> ;
    dcat:landingPage "https://www.legislation.gov.au/F2021L00319/2024-04-30/2024-04-30/text/original/epub/OEBPS/document_1/document_1.html#_Toc166157910"^^xsd:anyURI ;
    dcat:theme legcons:Item .

F2021L00319:79 a legcons:Item,
        owl:Class,
        dcat:Resource ;
    rdfs:label "Item - I79 5 2  Purpose of this Division"@en-AU ;
    dct:isPartOf F2021L00319:78 ;
    dct:isReferencedBy F2021L00319: ;
    rdfs:comment "5 2  Purpose of this Division - Abrievated Graph Key: I79"@en-AU ;
    skos:definition "5 2  Purpose of this Division"@en-AU ;
    skos:narrower F2021L00319:78 ;
    skos:prefLabel "Item I79"@en-AU ;
    dcat:accessURL <https://www.legislation.gov.au/F2021L00319/2024-04-30/2024-04-30/text/original/epub/OEBPS/document_1/document_1.html#_Toc166157912> ;
    dcat:landingPage "https://www.legislation.gov.au/F2021L00319/2024-04-30/2024-04-30/text/original/epub/OEBPS/document_1/document_1.html#_Toc166157912"^^xsd:anyURI ;
    dcat:theme legcons:Item .

F2021L00319:8 a legcons:Item,
        owl:Class,
        dcat:Resource ;
    rdfs:label "Item - I8 1 6  Definitions"@en-AU ;
    dct:isPartOf F2021L00319:1 ;
    dct:isReferencedBy F2021L00319: ;
    rdfs:comment "1 6  Definitions - Abrievated Graph Key: I8"@en-AU ;
    skos:definition "1 6  Definitions"@en-AU ;
    skos:narrower F2021L00319:1 ;
    skos:prefLabel "Item I8"@en-AU ;
    dcat:accessURL <https://www.legislation.gov.au/F2021L00319/2024-04-30/2024-04-30/text/original/epub/OEBPS/document_1/document_1.html#_Toc166157841> ;
    dcat:landingPage "https://www.legislation.gov.au/F2021L00319/2024-04-30/2024-04-30/text/original/epub/OEBPS/document_1/document_1.html#_Toc166157841"^^xsd:anyURI ;
    dcat:theme legcons:Item .

F2021L00319:80 a legcons:Item,
        owl:Class,
        dcat:Resource ;
    rdfs:label "Item - I80 5 3  Information for occupier of registered establishment where prescribed livestock are to be prepared for export by sea or air"@en-AU ;
    dct:isPartOf F2021L00319:78 ;
    dct:isReferencedBy F2021L00319: ;
    rdfs:comment "5 3  Information for occupier of registered establishment where prescribed livestock are to be prepared for export by sea or air - Abrievated Graph Key: I80"@en-AU ;
    skos:definition "5 3  Information for occupier of registered establishment where prescribed livestock are to be prepared for export by sea or air"@en-AU ;
    skos:narrower F2021L00319:78 ;
    skos:prefLabel "Item I80"@en-AU ;
    dcat:accessURL <https://www.legislation.gov.au/F2021L00319/2024-04-30/2024-04-30/text/original/epub/OEBPS/document_1/document_1.html#_Toc166157913> ;
    dcat:landingPage "https://www.legislation.gov.au/F2021L00319/2024-04-30/2024-04-30/text/original/epub/OEBPS/document_1/document_1.html#_Toc166157913"^^xsd:anyURI ;
    dcat:theme legcons:Item .

F2021L00319:81 a legcons:Item,
        owl:Class,
        dcat:Resource ;
    rdfs:label "Item - I81 5 4  Information for occupier of approved premises where prescribed livestock are to be prepared for export by air"@en-AU ;
    dct:isPartOf F2021L00319:78 ;
    dct:isReferencedBy F2021L00319: ;
    rdfs:comment "5 4  Information for occupier of approved premises where prescribed livestock are to be prepared for export by air - Abrievated Graph Key: I81"@en-AU ;
    skos:definition "5 4  Information for occupier of approved premises where prescribed livestock are to be prepared for export by air"@en-AU ;
    skos:narrower F2021L00319:78 ;
    skos:prefLabel "Item I81"@en-AU ;
    dcat:accessURL <https://www.legislation.gov.au/F2021L00319/2024-04-30/2024-04-30/text/original/epub/OEBPS/document_1/document_1.html#_Toc166157914> ;
    dcat:landingPage "https://www.legislation.gov.au/F2021L00319/2024-04-30/2024-04-30/text/original/epub/OEBPS/document_1/document_1.html#_Toc166157914"^^xsd:anyURI ;
    dcat:theme legcons:Item .

F2021L00319:82 a legcons:Item,
        owl:Class,
        dcat:Resource ;
    rdfs:label "Item - I82 5 4 A  Importing country requirements must be met"@en-AU ;
    dct:isPartOf F2021L00319:78 ;
    dct:isReferencedBy F2021L00319: ;
    rdfs:comment "5 4 A  Importing country requirements must be met - Abrievated Graph Key: I82"@en-AU ;
    skos:definition "5 4 A  Importing country requirements must be met"@en-AU ;
    skos:narrower F2021L00319:78 ;
    skos:prefLabel "Item I82"@en-AU ;
    dcat:accessURL <https://www.legislation.gov.au/F2021L00319/2024-04-30/2024-04-30/text/original/epub/OEBPS/document_1/document_1.html#_Toc166157915> ;
    dcat:landingPage "https://www.legislation.gov.au/F2021L00319/2024-04-30/2024-04-30/text/original/epub/OEBPS/document_1/document_1.html#_Toc166157915"^^xsd:anyURI ;
    dcat:theme legcons:Item .

F2021L00319:83 a legcons:Item,
        owl:Class,
        dcat:Resource ;
    rdfs:label "Item - I83 5 4 B  Requirements of Australian Standards for the Export of Livestock must be met"@en-AU ;
    dct:isPartOf F2021L00319:78 ;
    dct:isReferencedBy F2021L00319: ;
    rdfs:comment "5 4 B  Requirements of Australian Standards for the Export of Livestock must be met - Abrievated Graph Key: I83"@en-AU ;
    skos:definition "5 4 B  Requirements of Australian Standards for the Export of Livestock must be met"@en-AU ;
    skos:narrower F2021L00319:78 ;
    skos:prefLabel "Item I83"@en-AU ;
    dcat:accessURL <https://www.legislation.gov.au/F2021L00319/2024-04-30/2024-04-30/text/original/epub/OEBPS/document_1/document_1.html#_Toc166157916> ;
    dcat:landingPage "https://www.legislation.gov.au/F2021L00319/2024-04-30/2024-04-30/text/original/epub/OEBPS/document_1/document_1.html#_Toc166157916"^^xsd:anyURI ;
    dcat:theme legcons:Item .

F2021L00319:85 a legcons:Item,
        owl:Class,
        dcat:Resource ;
    rdfs:label "Item - I85 5 5  Period within which application to renew approved arrangement must be made"@en-AU ;
    dct:isPartOf F2021L00319:84 ;
    dct:isReferencedBy F2021L00319: ;
    rdfs:comment "5 5  Period within which application to renew approved arrangement must be made - Abrievated Graph Key: I85"@en-AU ;
    skos:definition "5 5  Period within which application to renew approved arrangement must be made"@en-AU ;
    skos:narrower F2021L00319:84 ;
    skos:prefLabel "Item I85"@en-AU ;
    dcat:accessURL <https://www.legislation.gov.au/F2021L00319/2024-04-30/2024-04-30/text/original/epub/OEBPS/document_1/document_1.html#_Toc166157918> ;
    dcat:landingPage "https://www.legislation.gov.au/F2021L00319/2024-04-30/2024-04-30/text/original/epub/OEBPS/document_1/document_1.html#_Toc166157918"^^xsd:anyURI ;
    dcat:theme legcons:Item .

F2021L00319:87 a legcons:Item,
        owl:Class,
        dcat:Resource ;
    rdfs:label "Item - I87 5 6  Application by holder for variationgrounds for refusing application"@en-AU ;
    dct:isPartOf F2021L00319:86 ;
    dct:isReferencedBy F2021L00319: ;
    rdfs:comment "5 6  Application by holder for variationgrounds for refusing application - Abrievated Graph Key: I87"@en-AU ;
    skos:definition "5 6  Application by holder for variationgrounds for refusing application"@en-AU ;
    skos:narrower F2021L00319:86 ;
    skos:prefLabel "Item I87"@en-AU ;
    dcat:accessURL <https://www.legislation.gov.au/F2021L00319/2024-04-30/2024-04-30/text/original/epub/OEBPS/document_1/document_1.html#_Toc166157920> ;
    dcat:landingPage "https://www.legislation.gov.au/F2021L00319/2024-04-30/2024-04-30/text/original/epub/OEBPS/document_1/document_1.html#_Toc166157920"^^xsd:anyURI ;
    dcat:theme legcons:Item .

F2021L00319:89 a legcons:Item,
        owl:Class,
        dcat:Resource ;
    rdfs:label "Item - I89 5 7  Other grounds for suspension"@en-AU ;
    dct:isPartOf F2021L00319:88 ;
    dct:isReferencedBy F2021L00319: ;
    rdfs:comment "5 7  Other grounds for suspension - Abrievated Graph Key: I89"@en-AU ;
    skos:definition "5 7  Other grounds for suspension"@en-AU ;
    skos:narrower F2021L00319:88 ;
    skos:prefLabel "Item I89"@en-AU ;
    dcat:accessURL <https://www.legislation.gov.au/F2021L00319/2024-04-30/2024-04-30/text/original/epub/OEBPS/document_1/document_1.html#_Toc166157922> ;
    dcat:landingPage "https://www.legislation.gov.au/F2021L00319/2024-04-30/2024-04-30/text/original/epub/OEBPS/document_1/document_1.html#_Toc166157922"^^xsd:anyURI ;
    dcat:theme legcons:Item .

F2021L00319:91 a legcons:Item,
        owl:Class,
        dcat:Resource ;
    rdfs:label "Item - I91 5 8  Other grounds for revocation"@en-AU ;
    dct:isPartOf F2021L00319:90 ;
    dct:isReferencedBy F2021L00319: ;
    rdfs:comment "5 8  Other grounds for revocation - Abrievated Graph Key: I91"@en-AU ;
    skos:definition "5 8  Other grounds for revocation"@en-AU ;
    skos:narrower F2021L00319:90 ;
    skos:prefLabel "Item I91"@en-AU ;
    dcat:accessURL <https://www.legislation.gov.au/F2021L00319/2024-04-30/2024-04-30/text/original/epub/OEBPS/document_1/document_1.html#_Toc166157924> ;
    dcat:landingPage "https://www.legislation.gov.au/F2021L00319/2024-04-30/2024-04-30/text/original/epub/OEBPS/document_1/document_1.html#_Toc166157924"^^xsd:anyURI ;
    dcat:theme legcons:Item .

F2021L00319:94 a legcons:Item,
        owl:Class,
        dcat:Resource ;
    rdfs:label "Item - I94 5 9  Purpose of this Division"@en-AU ;
    dct:isPartOf F2021L00319:93 ;
    dct:isReferencedBy F2021L00319: ;
    rdfs:comment "5 9  Purpose of this Division - Abrievated Graph Key: I94"@en-AU ;
    skos:definition "5 9  Purpose of this Division"@en-AU ;
    skos:narrower F2021L00319:93 ;
    skos:prefLabel "Item I94"@en-AU ;
    dcat:accessURL <https://www.legislation.gov.au/F2021L00319/2024-04-30/2024-04-30/text/original/epub/OEBPS/document_1/document_1.html#_Toc166157927> ;
    dcat:landingPage "https://www.legislation.gov.au/F2021L00319/2024-04-30/2024-04-30/text/original/epub/OEBPS/document_1/document_1.html#_Toc166157927"^^xsd:anyURI ;
    dcat:theme legcons:Item .

F2021L00319:95 a legcons:Item,
        owl:Class,
        dcat:Resource ;
    rdfs:label "Item - I95 5 10  Requirements relating to the applicant"@en-AU ;
    dct:isPartOf F2021L00319:93 ;
    dct:isReferencedBy F2021L00319: ;
    rdfs:comment "5 10  Requirements relating to the applicant - Abrievated Graph Key: I95"@en-AU ;
    skos:definition "5 10  Requirements relating to the applicant"@en-AU ;
    skos:narrower F2021L00319:93 ;
    skos:prefLabel "Item I95"@en-AU ;
    dcat:accessURL <https://www.legislation.gov.au/F2021L00319/2024-04-30/2024-04-30/text/original/epub/OEBPS/document_1/document_1.html#_Toc166157928> ;
    dcat:landingPage "https://www.legislation.gov.au/F2021L00319/2024-04-30/2024-04-30/text/original/epub/OEBPS/document_1/document_1.html#_Toc166157928"^^xsd:anyURI ;
    dcat:theme legcons:Item .

F2021L00319:96 a legcons:Item,
        owl:Class,
        dcat:Resource ;
    rdfs:label "Item - I96 5 11  Assurance rules and standards"@en-AU ;
    dct:isPartOf F2021L00319:93 ;
    dct:isReferencedBy F2021L00319: ;
    rdfs:comment "5 11  Assurance rules and standards - Abrievated Graph Key: I96"@en-AU ;
    skos:definition "5 11  Assurance rules and standards"@en-AU ;
    skos:narrower F2021L00319:93 ;
    skos:prefLabel "Item I96"@en-AU ;
    dcat:accessURL <https://www.legislation.gov.au/F2021L00319/2024-04-30/2024-04-30/text/original/epub/OEBPS/document_1/document_1.html#_Toc166157929> ;
    dcat:landingPage "https://www.legislation.gov.au/F2021L00319/2024-04-30/2024-04-30/text/original/epub/OEBPS/document_1/document_1.html#_Toc166157929"^^xsd:anyURI ;
    dcat:theme legcons:Item .

F2021L00319:97 a legcons:Item,
        owl:Class,
        dcat:Resource ;
    rdfs:label "Item - I97 5 12  Applicants management practices and business structure etc"@en-AU ;
    dct:isPartOf F2021L00319:93 ;
    dct:isReferencedBy F2021L00319: ;
    rdfs:comment "5 12  Applicants management practices and business structure etc - Abrievated Graph Key: I97"@en-AU ;
    skos:definition "5 12  Applicants management practices and business structure etc"@en-AU ;
    skos:narrower F2021L00319:93 ;
    skos:prefLabel "Item I97"@en-AU ;
    dcat:accessURL <https://www.legislation.gov.au/F2021L00319/2024-04-30/2024-04-30/text/original/epub/OEBPS/document_1/document_1.html#_Toc166157930> ;
    dcat:landingPage "https://www.legislation.gov.au/F2021L00319/2024-04-30/2024-04-30/text/original/epub/OEBPS/document_1/document_1.html#_Toc166157930"^^xsd:anyURI ;
    dcat:theme legcons:Item .

F2021L00319:98 a legcons:Item,
        owl:Class,
        dcat:Resource ;
    rdfs:label "Item - I98 5 13  Kinds of prescribed livestock and countries in relation to which exporter supply chain assurance operations are to be carried out"@en-AU ;
    dct:isPartOf F2021L00319:93 ;
    dct:isReferencedBy F2021L00319: ;
    rdfs:comment "5 13  Kinds of prescribed livestock and countries in relation to which exporter supply chain assurance operations are to be carried out - Abrievated Graph Key: I98"@en-AU ;
    skos:definition "5 13  Kinds of prescribed livestock and countries in relation to which exporter supply chain assurance operations are to be carried out"@en-AU ;
    skos:narrower F2021L00319:93 ;
    skos:prefLabel "Item I98"@en-AU ;
    dcat:accessURL <https://www.legislation.gov.au/F2021L00319/2024-04-30/2024-04-30/text/original/epub/OEBPS/document_1/document_1.html#_Toc166157931> ;
    dcat:landingPage "https://www.legislation.gov.au/F2021L00319/2024-04-30/2024-04-30/text/original/epub/OEBPS/document_1/document_1.html#_Toc166157931"^^xsd:anyURI ;
    dcat:theme legcons:Item .

F2021L00319:105 a legcons:Division,
        owl:Class,
        dcat:Resource ;
    rdfs:label "Division - D105 Division 3 Renewal of approved arrangement"@en-AU ;
    dct:hasPart F2021L00319:106 ;
    dct:isPartOf F2021L00319:92 ;
    dct:isReferencedBy F2021L00319: ;
    rdfs:comment "Division 3 Renewal of approved arrangement - Abrievated Graph Key: D105"@en-AU ;
    skos:broader F2021L00319:106 ;
    skos:definition "Division 3 Renewal of approved arrangement"@en-AU ;
    skos:narrower F2021L00319:92 ;
    skos:prefLabel "Division D105"@en-AU ;
    dcat:accessURL <https://www.legislation.gov.au/F2021L00319/2024-04-30/2024-04-30/text/original/epub/OEBPS/document_1/document_1.html#_Toc166157938> ;
    dcat:landingPage "https://www.legislation.gov.au/F2021L00319/2024-04-30/2024-04-30/text/original/epub/OEBPS/document_1/document_1.html#_Toc166157938"^^xsd:anyURI ;
    dcat:theme legcons:Division .

F2021L00319:11 a legcons:Division,
        owl:Class,
        dcat:Resource ;
    rdfs:label "Division - D11 Division 1 Prescribed goods"@en-AU ;
    dct:hasPart F2021L00319:12 ;
    dct:isPartOf F2021L00319:10 ;
    dct:isReferencedBy F2021L00319: ;
    rdfs:comment "Division 1 Prescribed goods - Abrievated Graph Key: D11"@en-AU ;
    skos:broader F2021L00319:12 ;
    skos:definition "Division 1 Prescribed goods"@en-AU ;
    skos:narrower F2021L00319:10 ;
    skos:prefLabel "Division D11"@en-AU ;
    dcat:accessURL <https://www.legislation.gov.au/F2021L00319/2024-04-30/2024-04-30/text/original/epub/OEBPS/document_1/document_1.html#_Toc166157844> ;
    dcat:landingPage "https://www.legislation.gov.au/F2021L00319/2024-04-30/2024-04-30/text/original/epub/OEBPS/document_1/document_1.html#_Toc166157844"^^xsd:anyURI ;
    dcat:theme legcons:Division .

F2021L00319:114 a legcons:Division,
        owl:Class,
        dcat:Resource ;
    rdfs:label "Division - D114 Division 6 Revocation of approved arrangement"@en-AU ;
    dct:hasPart F2021L00319:115 ;
    dct:isPartOf F2021L00319:92 ;
    dct:isReferencedBy F2021L00319: ;
    rdfs:comment "Division 6 Revocation of approved arrangement - Abrievated Graph Key: D114"@en-AU ;
    skos:broader F2021L00319:115 ;
    skos:definition "Division 6 Revocation of approved arrangement"@en-AU ;
    skos:narrower F2021L00319:92 ;
    skos:prefLabel "Division D114"@en-AU ;
    dcat:accessURL <https://www.legislation.gov.au/F2021L00319/2024-04-30/2024-04-30/text/original/epub/OEBPS/document_1/document_1.html#_Toc166157947> ;
    dcat:landingPage "https://www.legislation.gov.au/F2021L00319/2024-04-30/2024-04-30/text/original/epub/OEBPS/document_1/document_1.html#_Toc166157947"^^xsd:anyURI ;
    dcat:theme legcons:Division .

F2021L00319:116 a legcons:Division,
        owl:Class,
        dcat:Resource ;
    rdfs:label "Division - D116 Division 7 Fit and proper persons"@en-AU ;
    dct:hasPart F2021L00319:117 ;
    dct:isPartOf F2021L00319:92 ;
    dct:isReferencedBy F2021L00319: ;
    rdfs:comment "Division 7 Fit and proper persons - Abrievated Graph Key: D116"@en-AU ;
    skos:broader F2021L00319:117 ;
    skos:definition "Division 7 Fit and proper persons"@en-AU ;
    skos:narrower F2021L00319:92 ;
    skos:prefLabel "Division D116"@en-AU ;
    dcat:accessURL <https://www.legislation.gov.au/F2021L00319/2024-04-30/2024-04-30/text/original/epub/OEBPS/document_1/document_1.html#_Toc166157949> ;
    dcat:landingPage "https://www.legislation.gov.au/F2021L00319/2024-04-30/2024-04-30/text/original/epub/OEBPS/document_1/document_1.html#_Toc166157949"^^xsd:anyURI ;
    dcat:theme legcons:Division .

F2021L00319:118 a legcons:Division,
        owl:Class,
        dcat:Resource ;
    rdfs:label "Division - D118 Division 8 Miscellaneous"@en-AU ;
    dct:hasPart F2021L00319:119 ;
    dct:isPartOf F2021L00319:92 ;
    dct:isReferencedBy F2021L00319: ;
    rdfs:comment "Division 8 Miscellaneous - Abrievated Graph Key: D118"@en-AU ;
    skos:broader F2021L00319:119 ;
    skos:definition "Division 8 Miscellaneous"@en-AU ;
    skos:narrower F2021L00319:92 ;
    skos:prefLabel "Division D118"@en-AU ;
    dcat:accessURL <https://www.legislation.gov.au/F2021L00319/2024-04-30/2024-04-30/text/original/epub/OEBPS/document_1/document_1.html#_Toc166157951> ;
    dcat:landingPage "https://www.legislation.gov.au/F2021L00319/2024-04-30/2024-04-30/text/original/epub/OEBPS/document_1/document_1.html#_Toc166157951"^^xsd:anyURI ;
    dcat:theme legcons:Division .

F2021L00319:127 a legcons:Division,
        owl:Class,
        dcat:Resource ;
    rdfs:label "Division - D127 Division 1 Requirements for grant of livestock export licence"@en-AU ;
    dct:hasPart F2021L00319:128 ;
    dct:isPartOf F2021L00319:126 ;
    dct:isReferencedBy F2021L00319: ;
    rdfs:comment "Division 1 Requirements for grant of livestock export licence - Abrievated Graph Key: D127"@en-AU ;
    skos:broader F2021L00319:128 ;
    skos:definition "Division 1 Requirements for grant of livestock export licence"@en-AU ;
    skos:narrower F2021L00319:126 ;
    skos:prefLabel "Division D127"@en-AU ;
    dcat:accessURL <https://www.legislation.gov.au/F2021L00319/2024-04-30/2024-04-30/text/original/epub/OEBPS/document_1/document_1.html#_Toc166157960> ;
    dcat:landingPage "https://www.legislation.gov.au/F2021L00319/2024-04-30/2024-04-30/text/original/epub/OEBPS/document_1/document_1.html#_Toc166157960"^^xsd:anyURI ;
    dcat:theme legcons:Division .

F2021L00319:133 a legcons:Division,
        owl:Class,
        dcat:Resource ;
    rdfs:label "Division - D133 Division 1 Purpose of this Part"@en-AU ;
    dct:hasPart F2021L00319:134 ;
    dct:isPartOf F2021L00319:132 ;
    dct:isReferencedBy F2021L00319: ;
    rdfs:comment "Division 1 Purpose of this Part - Abrievated Graph Key: D133"@en-AU ;
    skos:broader F2021L00319:134 ;
    skos:definition "Division 1 Purpose of this Part"@en-AU ;
    skos:narrower F2021L00319:132 ;
    skos:prefLabel "Division D133"@en-AU ;
    dcat:accessURL <https://www.legislation.gov.au/F2021L00319/2024-04-30/2024-04-30/text/original/epub/OEBPS/document_1/document_1.html#_Toc166157966> ;
    dcat:landingPage "https://www.legislation.gov.au/F2021L00319/2024-04-30/2024-04-30/text/original/epub/OEBPS/document_1/document_1.html#_Toc166157966"^^xsd:anyURI ;
    dcat:theme legcons:Division .

F2021L00319:145 a legcons:Subdivision,
        owl:Class,
        dcat:Resource ;
    rdfs:label "Subdivision - S145 Subdivision AApplication of this Division"@en-AU ;
    dct:hasPart F2021L00319:146 ;
    dct:isPartOf F2021L00319:144 ;
    dct:isReferencedBy F2021L00319: ;
    rdfs:comment "Subdivision AApplication of this Division - Abrievated Graph Key: S145"@en-AU ;
    skos:broader F2021L00319:146 ;
    skos:definition "Subdivision AApplication of this Division"@en-AU ;
    skos:narrower F2021L00319:144 ;
    skos:prefLabel "Subdivision S145"@en-AU ;
    dcat:accessURL <https://www.legislation.gov.au/F2021L00319/2024-04-30/2024-04-30/text/original/epub/OEBPS/document_1/document_1.html#_Toc166157978> ;
    dcat:landingPage "https://www.legislation.gov.au/F2021L00319/2024-04-30/2024-04-30/text/original/epub/OEBPS/document_1/document_1.html#_Toc166157978"^^xsd:anyURI ;
    dcat:theme legcons:Subdivision .

F2021L00319:196 a legcons:Division,
        owl:Class,
        dcat:Resource ;
    rdfs:label "Division - D196 Division 4 Other matters"@en-AU ;
    dct:hasPart F2021L00319:197 ;
    dct:isPartOf F2021L00319:125 ;
    dct:isReferencedBy F2021L00319: ;
    rdfs:comment "Division 4 Other matters - Abrievated Graph Key: D196"@en-AU ;
    skos:broader F2021L00319:197 ;
    skos:definition "Division 4 Other matters"@en-AU ;
    skos:narrower F2021L00319:125 ;
    skos:prefLabel "Division D196"@en-AU ;
    dcat:accessURL <https://www.legislation.gov.au/F2021L00319/2024-04-30/2024-04-30/text/original/epub/OEBPS/document_1/document_1.html#_Toc166158029> ;
    dcat:landingPage "https://www.legislation.gov.au/F2021L00319/2024-04-30/2024-04-30/text/original/epub/OEBPS/document_1/document_1.html#_Toc166158029"^^xsd:anyURI ;
    dcat:theme legcons:Division .

F2021L00319:215 a legcons:Chapter,
        owl:Class,
        dcat:Resource ;
    rdfs:label "Chapter - C215 Chapter 8 Other matters relating to export"@en-AU ;
    dct:hasPart F2021L00319:216,
        F2021L00319:235 ;
    dct:isReferencedBy F2021L00319: ;
    rdfs:comment "Chapter 8 Other matters relating to export - Abrievated Graph Key: C215"@en-AU ;
    skos:broader F2021L00319:216,
        F2021L00319:235 ;
    skos:definition "Chapter 8 Other matters relating to export"@en-AU ;
    skos:prefLabel "Chapter C215"@en-AU ;
    dcat:accessURL <https://www.legislation.gov.au/F2021L00319/2024-04-30/2024-04-30/text/original/epub/OEBPS/document_1/document_1.html#_Toc166158048> ;
    dcat:landingPage "https://www.legislation.gov.au/F2021L00319/2024-04-30/2024-04-30/text/original/epub/OEBPS/document_1/document_1.html#_Toc166158048"^^xsd:anyURI ;
    dcat:theme legcons:Chapter .

F2021L00319:264 a legcons:Division,
        owl:Class,
        dcat:Resource ;
    rdfs:label "Division - D264 Division 1 General"@en-AU ;
    dct:hasPart F2021L00319:265 ;
    dct:isPartOf F2021L00319:263 ;
    dct:isReferencedBy F2021L00319: ;
    rdfs:comment "Division 1 General - Abrievated Graph Key: D264"@en-AU ;
    skos:broader F2021L00319:265 ;
    skos:definition "Division 1 General"@en-AU ;
    skos:narrower F2021L00319:263 ;
    skos:prefLabel "Division D264"@en-AU ;
    dcat:accessURL <https://www.legislation.gov.au/F2021L00319/2024-04-30/2024-04-30/text/original/epub/OEBPS/document_1/document_1.html#_Toc166158097> ;
    dcat:landingPage "https://www.legislation.gov.au/F2021L00319/2024-04-30/2024-04-30/text/original/epub/OEBPS/document_1/document_1.html#_Toc166158097"^^xsd:anyURI ;
    dcat:theme legcons:Division .

F2021L00319:272 a legcons:Division,
        owl:Class,
        dcat:Resource ;
    rdfs:label "Division - D272 Division 1 General"@en-AU ;
    dct:hasPart F2021L00319:273 ;
    dct:isPartOf F2021L00319:271 ;
    dct:isReferencedBy F2021L00319: ;
    rdfs:comment "Division 1 General - Abrievated Graph Key: D272"@en-AU ;
    skos:broader F2021L00319:273 ;
    skos:definition "Division 1 General"@en-AU ;
    skos:narrower F2021L00319:271 ;
    skos:prefLabel "Division D272"@en-AU ;
    dcat:accessURL <https://www.legislation.gov.au/F2021L00319/2024-04-30/2024-04-30/text/original/epub/OEBPS/document_1/document_1.html#_Toc166158105> ;
    dcat:landingPage "https://www.legislation.gov.au/F2021L00319/2024-04-30/2024-04-30/text/original/epub/OEBPS/document_1/document_1.html#_Toc166158105"^^xsd:anyURI ;
    dcat:theme legcons:Division .

F2021L00319:278 a legcons:Division,
        owl:Class,
        dcat:Resource ;
    rdfs:label "Division - D278 Division 1 Purpose of this Part"@en-AU ;
    dct:hasPart F2021L00319:279 ;
    dct:isPartOf F2021L00319:277 ;
    dct:isReferencedBy F2021L00319: ;
    rdfs:comment "Division 1 Purpose of this Part - Abrievated Graph Key: D278"@en-AU ;
    skos:broader F2021L00319:279 ;
    skos:definition "Division 1 Purpose of this Part"@en-AU ;
    skos:narrower F2021L00319:277 ;
    skos:prefLabel "Division D278"@en-AU ;
    dcat:accessURL <https://www.legislation.gov.au/F2021L00319/2024-04-30/2024-04-30/text/original/epub/OEBPS/document_1/document_1.html#_Toc166158111> ;
    dcat:landingPage "https://www.legislation.gov.au/F2021L00319/2024-04-30/2024-04-30/text/original/epub/OEBPS/document_1/document_1.html#_Toc166158111"^^xsd:anyURI ;
    dcat:theme legcons:Division .

F2021L00319:304 a legcons:Division,
        owl:Class,
        dcat:Resource ;
    rdfs:label "Division - D304 Division 8 Fit and proper persons"@en-AU ;
    dct:hasPart F2021L00319:305 ;
    dct:isPartOf F2021L00319:277 ;
    dct:isReferencedBy F2021L00319: ;
    rdfs:comment "Division 8 Fit and proper persons - Abrievated Graph Key: D304"@en-AU ;
    skos:broader F2021L00319:305 ;
    skos:definition "Division 8 Fit and proper persons"@en-AU ;
    skos:narrower F2021L00319:277 ;
    skos:prefLabel "Division D304"@en-AU ;
    dcat:accessURL <https://www.legislation.gov.au/F2021L00319/2024-04-30/2024-04-30/text/original/epub/OEBPS/document_1/document_1.html#_Toc166158137> ;
    dcat:landingPage "https://www.legislation.gov.au/F2021L00319/2024-04-30/2024-04-30/text/original/epub/OEBPS/document_1/document_1.html#_Toc166158137"^^xsd:anyURI ;
    dcat:theme legcons:Division .

F2021L00319:311 a legcons:Division,
        owl:Class,
        dcat:Resource ;
    rdfs:label "Division - D311 Division 1 Purpose of this Part"@en-AU ;
    dct:hasPart F2021L00319:312 ;
    dct:isPartOf F2021L00319:310 ;
    dct:isReferencedBy F2021L00319: ;
    rdfs:comment "Division 1 Purpose of this Part - Abrievated Graph Key: D311"@en-AU ;
    skos:broader F2021L00319:312 ;
    skos:definition "Division 1 Purpose of this Part"@en-AU ;
    skos:narrower F2021L00319:310 ;
    skos:prefLabel "Division D311"@en-AU ;
    dcat:accessURL <https://www.legislation.gov.au/F2021L00319/2024-04-30/2024-04-30/text/original/epub/OEBPS/document_1/document_1.html#_Toc166158144> ;
    dcat:landingPage "https://www.legislation.gov.au/F2021L00319/2024-04-30/2024-04-30/text/original/epub/OEBPS/document_1/document_1.html#_Toc166158144"^^xsd:anyURI ;
    dcat:theme legcons:Division .

F2021L00319:329 a legcons:Subdivision,
        owl:Class,
        dcat:Resource ;
    rdfs:label "Subdivision - S329 Subdivision ECopies of approved export program"@en-AU ;
    dct:hasPart F2021L00319:330 ;
    dct:isPartOf F2021L00319:313 ;
    dct:isReferencedBy F2021L00319: ;
    rdfs:comment "Subdivision ECopies of approved export program - Abrievated Graph Key: S329"@en-AU ;
    skos:broader F2021L00319:330 ;
    skos:definition "Subdivision ECopies of approved export program"@en-AU ;
    skos:narrower F2021L00319:313 ;
    skos:prefLabel "Subdivision S329"@en-AU ;
    dcat:accessURL <https://www.legislation.gov.au/F2021L00319/2024-04-30/2024-04-30/text/original/epub/OEBPS/document_1/document_1.html#_Toc166158162> ;
    dcat:landingPage "https://www.legislation.gov.au/F2021L00319/2024-04-30/2024-04-30/text/original/epub/OEBPS/document_1/document_1.html#_Toc166158162"^^xsd:anyURI ;
    dcat:theme legcons:Subdivision .

F2021L00319:347 a legcons:Chapter,
        owl:Class,
        dcat:Resource ;
    rdfs:label "Chapter - C347 Chapter 10 Compliance and enforcement"@en-AU ;
    dct:hasPart F2021L00319:348,
        F2021L00319:349 ;
    dct:isReferencedBy F2021L00319: ;
    rdfs:comment "Chapter 10 Compliance and enforcement - Abrievated Graph Key: C347"@en-AU ;
    skos:broader F2021L00319:348,
        F2021L00319:349 ;
    skos:definition "Chapter 10 Compliance and enforcement"@en-AU ;
    skos:prefLabel "Chapter C347"@en-AU ;
    dcat:accessURL <https://www.legislation.gov.au/F2021L00319/2024-04-30/2024-04-30/text/original/epub/OEBPS/document_1/document_1.html#_Toc166158180> ;
    dcat:landingPage "https://www.legislation.gov.au/F2021L00319/2024-04-30/2024-04-30/text/original/epub/OEBPS/document_1/document_1.html#_Toc166158180"^^xsd:anyURI ;
    dcat:theme legcons:Chapter .

F2021L00319:351 a legcons:Part,
        owl:Class,
        dcat:Resource ;
    rdfs:label "Part - P351 Part 1 Review of decisions"@en-AU ;
    dct:hasPart F2021L00319:352 ;
    dct:isPartOf F2021L00319:350 ;
    dct:isReferencedBy F2021L00319: ;
    rdfs:comment "Part 1 Review of decisions - Abrievated Graph Key: P351"@en-AU ;
    skos:broader F2021L00319:352 ;
    skos:definition "Part 1 Review of decisions"@en-AU ;
    skos:narrower F2021L00319:350 ;
    skos:prefLabel "Part P351"@en-AU ;
    dcat:accessURL <https://www.legislation.gov.au/F2021L00319/2024-04-30/2024-04-30/text/original/epub/OEBPS/document_1/document_1.html#_Toc166158184> ;
    dcat:landingPage "https://www.legislation.gov.au/F2021L00319/2024-04-30/2024-04-30/text/original/epub/OEBPS/document_1/document_1.html#_Toc166158184"^^xsd:anyURI ;
    dcat:theme legcons:Part .

F2021L00319:364 a legcons:Part,
        owl:Class,
        dcat:Resource ;
    rdfs:label "Part - P364 Part 3 Samples"@en-AU ;
    dct:hasPart F2021L00319:365 ;
    dct:isPartOf F2021L00319:350 ;
    dct:isReferencedBy F2021L00319: ;
    rdfs:comment "Part 3 Samples - Abrievated Graph Key: P364"@en-AU ;
    skos:broader F2021L00319:365 ;
    skos:definition "Part 3 Samples"@en-AU ;
    skos:narrower F2021L00319:350 ;
    skos:prefLabel "Part P364"@en-AU ;
    dcat:accessURL <https://www.legislation.gov.au/F2021L00319/2024-04-30/2024-04-30/text/original/epub/OEBPS/document_1/document_1.html#_Toc166158197> ;
    dcat:landingPage "https://www.legislation.gov.au/F2021L00319/2024-04-30/2024-04-30/text/original/epub/OEBPS/document_1/document_1.html#_Toc166158197"^^xsd:anyURI ;
    dcat:theme legcons:Part .

F2021L00319:369 a legcons:Part,
        owl:Class,
        dcat:Resource ;
    rdfs:label "Part - P369 Part 5 Relevant Commonwealth liabilities"@en-AU ;
    dct:hasPart F2021L00319:370 ;
    dct:isPartOf F2021L00319:350 ;
    dct:isReferencedBy F2021L00319: ;
    rdfs:comment "Part 5 Relevant Commonwealth liabilities - Abrievated Graph Key: P369"@en-AU ;
    skos:broader F2021L00319:370 ;
    skos:definition "Part 5 Relevant Commonwealth liabilities"@en-AU ;
    skos:narrower F2021L00319:350 ;
    skos:prefLabel "Part P369"@en-AU ;
    dcat:accessURL <https://www.legislation.gov.au/F2021L00319/2024-04-30/2024-04-30/text/original/epub/OEBPS/document_1/document_1.html#_Toc166158202> ;
    dcat:landingPage "https://www.legislation.gov.au/F2021L00319/2024-04-30/2024-04-30/text/original/epub/OEBPS/document_1/document_1.html#_Toc166158202"^^xsd:anyURI ;
    dcat:theme legcons:Part .

F2021L00319:371 a legcons:Part,
        owl:Class,
        dcat:Resource ;
    rdfs:label "Part - P371 Part 6 Miscellaneous"@en-AU ;
    dct:hasPart F2021L00319:372 ;
    dct:isPartOf F2021L00319:350 ;
    dct:isReferencedBy F2021L00319: ;
    rdfs:comment "Part 6 Miscellaneous - Abrievated Graph Key: P371"@en-AU ;
    skos:broader F2021L00319:372 ;
    skos:definition "Part 6 Miscellaneous"@en-AU ;
    skos:narrower F2021L00319:350 ;
    skos:prefLabel "Part P371"@en-AU ;
    dcat:accessURL <https://www.legislation.gov.au/F2021L00319/2024-04-30/2024-04-30/text/original/epub/OEBPS/document_1/document_1.html#_Toc166158204> ;
    dcat:landingPage "https://www.legislation.gov.au/F2021L00319/2024-04-30/2024-04-30/text/original/epub/OEBPS/document_1/document_1.html#_Toc166158204"^^xsd:anyURI ;
    dcat:theme legcons:Part .

F2021L00319:374 a legcons:Part,
        owl:Class,
        dcat:Resource ;
    rdfs:label "Part - P374 Part 1 Preliminary"@en-AU ;
    dct:hasPart F2021L00319:375 ;
    dct:isPartOf F2021L00319:373 ;
    dct:isReferencedBy F2021L00319: ;
    rdfs:comment "Part 1 Preliminary - Abrievated Graph Key: P374"@en-AU ;
    skos:broader F2021L00319:375 ;
    skos:definition "Part 1 Preliminary"@en-AU ;
    skos:narrower F2021L00319:373 ;
    skos:prefLabel "Part P374"@en-AU ;
    dcat:accessURL <https://www.legislation.gov.au/F2021L00319/2024-04-30/2024-04-30/text/original/epub/OEBPS/document_1/document_1.html#_Toc166158207> ;
    dcat:landingPage "https://www.legislation.gov.au/F2021L00319/2024-04-30/2024-04-30/text/original/epub/OEBPS/document_1/document_1.html#_Toc166158207"^^xsd:anyURI ;
    dcat:theme legcons:Part .

F2021L00319:417 a legcons:Part,
        owl:Class,
        dcat:Resource ;
    rdfs:label "Part - P417 Part 6 Amendments made by the Export Control Animals Amendment Northern Hemisphere Summer Prohibition Rules 2022"@en-AU ;
    dct:hasPart F2021L00319:418 ;
    dct:isPartOf F2021L00319:373 ;
    dct:isReferencedBy F2021L00319: ;
    rdfs:comment "Part 6 Amendments made by the Export Control Animals Amendment Northern Hemisphere Summer Prohibition Rules 2022 - Abrievated Graph Key: P417"@en-AU ;
    skos:broader F2021L00319:418 ;
    skos:definition "Part 6 Amendments made by the Export Control Animals Amendment Northern Hemisphere Summer Prohibition Rules 2022"@en-AU ;
    skos:narrower F2021L00319:373 ;
    skos:prefLabel "Part P417"@en-AU ;
    dcat:accessURL <https://www.legislation.gov.au/F2021L00319/2024-04-30/2024-04-30/text/original/epub/OEBPS/document_1/document_1.html#_Toc166158250> ;
    dcat:landingPage "https://www.legislation.gov.au/F2021L00319/2024-04-30/2024-04-30/text/original/epub/OEBPS/document_1/document_1.html#_Toc166158250"^^xsd:anyURI ;
    dcat:theme legcons:Part .

F2021L00319:419 a legcons:Part,
        owl:Class,
        dcat:Resource ;
    rdfs:label "Part - P419 Part 7 Amendments made by the Export Control Animals Amendment Northern Hemisphere Summer Conditions Rules 2023"@en-AU ;
    dct:hasPart F2021L00319:420 ;
    dct:isPartOf F2021L00319:373 ;
    dct:isReferencedBy F2021L00319: ;
    rdfs:comment "Part 7 Amendments made by the Export Control Animals Amendment Northern Hemisphere Summer Conditions Rules 2023 - Abrievated Graph Key: P419"@en-AU ;
    skos:broader F2021L00319:420 ;
    skos:definition "Part 7 Amendments made by the Export Control Animals Amendment Northern Hemisphere Summer Conditions Rules 2023"@en-AU ;
    skos:narrower F2021L00319:373 ;
    skos:prefLabel "Part P419"@en-AU ;
    dcat:accessURL <https://www.legislation.gov.au/F2021L00319/2024-04-30/2024-04-30/text/original/epub/OEBPS/document_1/document_1.html#_Toc166158252> ;
    dcat:landingPage "https://www.legislation.gov.au/F2021L00319/2024-04-30/2024-04-30/text/original/epub/OEBPS/document_1/document_1.html#_Toc166158252"^^xsd:anyURI ;
    dcat:theme legcons:Part .

F2021L00319:44 a legcons:Part,
        owl:Class,
        dcat:Resource ;
    rdfs:label "Part - P44 Part 1 Application of this Chapter"@en-AU ;
    dct:hasPart F2021L00319:45 ;
    dct:isPartOf F2021L00319:43 ;
    dct:isReferencedBy F2021L00319: ;
    rdfs:comment "Part 1 Application of this Chapter - Abrievated Graph Key: P44"@en-AU ;
    skos:broader F2021L00319:45 ;
    skos:definition "Part 1 Application of this Chapter"@en-AU ;
    skos:narrower F2021L00319:43 ;
    skos:prefLabel "Part P44"@en-AU ;
    dcat:accessURL <https://www.legislation.gov.au/F2021L00319/2024-04-30/2024-04-30/text/original/epub/OEBPS/document_1/document_1.html#_Toc166157877> ;
    dcat:landingPage "https://www.legislation.gov.au/F2021L00319/2024-04-30/2024-04-30/text/original/epub/OEBPS/document_1/document_1.html#_Toc166157877"^^xsd:anyURI ;
    dcat:theme legcons:Part .

F2021L00319:50 a legcons:Division,
        owl:Class,
        dcat:Resource ;
    rdfs:label "Division - D50 Division 2 Other matters relating to registration"@en-AU ;
    dct:hasPart F2021L00319:51 ;
    dct:isPartOf F2021L00319:46 ;
    dct:isReferencedBy F2021L00319: ;
    rdfs:comment "Division 2 Other matters relating to registration - Abrievated Graph Key: D50"@en-AU ;
    skos:broader F2021L00319:51 ;
    skos:definition "Division 2 Other matters relating to registration"@en-AU ;
    skos:narrower F2021L00319:46 ;
    skos:prefLabel "Division D50"@en-AU ;
    dcat:accessURL <https://www.legislation.gov.au/F2021L00319/2024-04-30/2024-04-30/text/original/epub/OEBPS/document_1/document_1.html#_Toc166157883> ;
    dcat:landingPage "https://www.legislation.gov.au/F2021L00319/2024-04-30/2024-04-30/text/original/epub/OEBPS/document_1/document_1.html#_Toc166157883"^^xsd:anyURI ;
    dcat:theme legcons:Division .

F2021L00319:62 a legcons:Part,
        owl:Class,
        dcat:Resource ;
    rdfs:label "Part - P62 Part 5 Variation of registration"@en-AU ;
    dct:hasPart F2021L00319:63 ;
    dct:isPartOf F2021L00319:43 ;
    dct:isReferencedBy F2021L00319: ;
    rdfs:comment "Part 5 Variation of registration - Abrievated Graph Key: P62"@en-AU ;
    skos:broader F2021L00319:63 ;
    skos:definition "Part 5 Variation of registration"@en-AU ;
    skos:narrower F2021L00319:43 ;
    skos:prefLabel "Part P62"@en-AU ;
    dcat:accessURL <https://www.legislation.gov.au/F2021L00319/2024-04-30/2024-04-30/text/original/epub/OEBPS/document_1/document_1.html#_Toc166157895> ;
    dcat:landingPage "https://www.legislation.gov.au/F2021L00319/2024-04-30/2024-04-30/text/original/epub/OEBPS/document_1/document_1.html#_Toc166157895"^^xsd:anyURI ;
    dcat:theme legcons:Part .

F2021L00319:64 a legcons:Part,
        owl:Class,
        dcat:Resource ;
    rdfs:label "Part - P64 Part 6 Suspension of registration"@en-AU ;
    dct:hasPart F2021L00319:65 ;
    dct:isPartOf F2021L00319:43 ;
    dct:isReferencedBy F2021L00319: ;
    rdfs:comment "Part 6 Suspension of registration - Abrievated Graph Key: P64"@en-AU ;
    skos:broader F2021L00319:65 ;
    skos:definition "Part 6 Suspension of registration"@en-AU ;
    skos:narrower F2021L00319:43 ;
    skos:prefLabel "Part P64"@en-AU ;
    dcat:accessURL <https://www.legislation.gov.au/F2021L00319/2024-04-30/2024-04-30/text/original/epub/OEBPS/document_1/document_1.html#_Toc166157897> ;
    dcat:landingPage "https://www.legislation.gov.au/F2021L00319/2024-04-30/2024-04-30/text/original/epub/OEBPS/document_1/document_1.html#_Toc166157897"^^xsd:anyURI ;
    dcat:theme legcons:Part .

F2021L00319:66 a legcons:Part,
        owl:Class,
        dcat:Resource ;
    rdfs:label "Part - P66 Part 7 Revocation of registration"@en-AU ;
    dct:hasPart F2021L00319:67 ;
    dct:isPartOf F2021L00319:43 ;
    dct:isReferencedBy F2021L00319: ;
    rdfs:comment "Part 7 Revocation of registration - Abrievated Graph Key: P66"@en-AU ;
    skos:broader F2021L00319:67 ;
    skos:definition "Part 7 Revocation of registration"@en-AU ;
    skos:narrower F2021L00319:43 ;
    skos:prefLabel "Part P66"@en-AU ;
    dcat:accessURL <https://www.legislation.gov.au/F2021L00319/2024-04-30/2024-04-30/text/original/epub/OEBPS/document_1/document_1.html#_Toc166157899> ;
    dcat:landingPage "https://www.legislation.gov.au/F2021L00319/2024-04-30/2024-04-30/text/original/epub/OEBPS/document_1/document_1.html#_Toc166157899"^^xsd:anyURI ;
    dcat:theme legcons:Part .

F2021L00319:72 a legcons:Part,
        owl:Class,
        dcat:Resource ;
    rdfs:label "Part - P72 Part 9 Miscellaneous"@en-AU ;
    dct:hasPart F2021L00319:73 ;
    dct:isPartOf F2021L00319:43 ;
    dct:isReferencedBy F2021L00319: ;
    rdfs:comment "Part 9 Miscellaneous - Abrievated Graph Key: P72"@en-AU ;
    skos:broader F2021L00319:73 ;
    skos:definition "Part 9 Miscellaneous"@en-AU ;
    skos:narrower F2021L00319:43 ;
    skos:prefLabel "Part P72"@en-AU ;
    dcat:accessURL <https://www.legislation.gov.au/F2021L00319/2024-04-30/2024-04-30/text/original/epub/OEBPS/document_1/document_1.html#_Toc166157905> ;
    dcat:landingPage "https://www.legislation.gov.au/F2021L00319/2024-04-30/2024-04-30/text/original/epub/OEBPS/document_1/document_1.html#_Toc166157905"^^xsd:anyURI ;
    dcat:theme legcons:Part .

F2021L00319:76 a legcons:Division,
        owl:Class,
        dcat:Resource ;
    rdfs:label "Division - D76 Division 1 Requirements for approval"@en-AU ;
    dct:hasPart F2021L00319:77 ;
    dct:isPartOf F2021L00319:75 ;
    dct:isReferencedBy F2021L00319: ;
    rdfs:comment "Division 1 Requirements for approval - Abrievated Graph Key: D76"@en-AU ;
    skos:broader F2021L00319:77 ;
    skos:definition "Division 1 Requirements for approval"@en-AU ;
    skos:narrower F2021L00319:75 ;
    skos:prefLabel "Division D76"@en-AU ;
    dcat:accessURL <https://www.legislation.gov.au/F2021L00319/2024-04-30/2024-04-30/text/original/epub/OEBPS/document_1/document_1.html#_Toc166157909> ;
    dcat:landingPage "https://www.legislation.gov.au/F2021L00319/2024-04-30/2024-04-30/text/original/epub/OEBPS/document_1/document_1.html#_Toc166157909"^^xsd:anyURI ;
    dcat:theme legcons:Division .

F2021L00319:84 a legcons:Division,
        owl:Class,
        dcat:Resource ;
    rdfs:label "Division - D84 Division 3 Renewal of approved arrangement"@en-AU ;
    dct:hasPart F2021L00319:85 ;
    dct:isPartOf F2021L00319:75 ;
    dct:isReferencedBy F2021L00319: ;
    rdfs:comment "Division 3 Renewal of approved arrangement - Abrievated Graph Key: D84"@en-AU ;
    skos:broader F2021L00319:85 ;
    skos:definition "Division 3 Renewal of approved arrangement"@en-AU ;
    skos:narrower F2021L00319:75 ;
    skos:prefLabel "Division D84"@en-AU ;
    dcat:accessURL <https://www.legislation.gov.au/F2021L00319/2024-04-30/2024-04-30/text/original/epub/OEBPS/document_1/document_1.html#_Toc166157917> ;
    dcat:landingPage "https://www.legislation.gov.au/F2021L00319/2024-04-30/2024-04-30/text/original/epub/OEBPS/document_1/document_1.html#_Toc166157917"^^xsd:anyURI ;
    dcat:theme legcons:Division .

F2021L00319:86 a legcons:Division,
        owl:Class,
        dcat:Resource ;
    rdfs:label "Division - D86 Division 4 Variation of approved arrangement"@en-AU ;
    dct:hasPart F2021L00319:87 ;
    dct:isPartOf F2021L00319:75 ;
    dct:isReferencedBy F2021L00319: ;
    rdfs:comment "Division 4 Variation of approved arrangement - Abrievated Graph Key: D86"@en-AU ;
    skos:broader F2021L00319:87 ;
    skos:definition "Division 4 Variation of approved arrangement"@en-AU ;
    skos:narrower F2021L00319:75 ;
    skos:prefLabel "Division D86"@en-AU ;
    dcat:accessURL <https://www.legislation.gov.au/F2021L00319/2024-04-30/2024-04-30/text/original/epub/OEBPS/document_1/document_1.html#_Toc166157919> ;
    dcat:landingPage "https://www.legislation.gov.au/F2021L00319/2024-04-30/2024-04-30/text/original/epub/OEBPS/document_1/document_1.html#_Toc166157919"^^xsd:anyURI ;
    dcat:theme legcons:Division .

F2021L00319:88 a legcons:Division,
        owl:Class,
        dcat:Resource ;
    rdfs:label "Division - D88 Division 5 Suspension of approved arrangement"@en-AU ;
    dct:hasPart F2021L00319:89 ;
    dct:isPartOf F2021L00319:75 ;
    dct:isReferencedBy F2021L00319: ;
    rdfs:comment "Division 5 Suspension of approved arrangement - Abrievated Graph Key: D88"@en-AU ;
    skos:broader F2021L00319:89 ;
    skos:definition "Division 5 Suspension of approved arrangement"@en-AU ;
    skos:narrower F2021L00319:75 ;
    skos:prefLabel "Division D88"@en-AU ;
    dcat:accessURL <https://www.legislation.gov.au/F2021L00319/2024-04-30/2024-04-30/text/original/epub/OEBPS/document_1/document_1.html#_Toc166157921> ;
    dcat:landingPage "https://www.legislation.gov.au/F2021L00319/2024-04-30/2024-04-30/text/original/epub/OEBPS/document_1/document_1.html#_Toc166157921"^^xsd:anyURI ;
    dcat:theme legcons:Division .

F2021L00319:90 a legcons:Division,
        owl:Class,
        dcat:Resource ;
    rdfs:label "Division - D90 Division 6 Revocation of approved arrangement"@en-AU ;
    dct:hasPart F2021L00319:91 ;
    dct:isPartOf F2021L00319:75 ;
    dct:isReferencedBy F2021L00319: ;
    rdfs:comment "Division 6 Revocation of approved arrangement - Abrievated Graph Key: D90"@en-AU ;
    skos:broader F2021L00319:91 ;
    skos:definition "Division 6 Revocation of approved arrangement"@en-AU ;
    skos:narrower F2021L00319:75 ;
    skos:prefLabel "Division D90"@en-AU ;
    dcat:accessURL <https://www.legislation.gov.au/F2021L00319/2024-04-30/2024-04-30/text/original/epub/OEBPS/document_1/document_1.html#_Toc166157923> ;
    dcat:landingPage "https://www.legislation.gov.au/F2021L00319/2024-04-30/2024-04-30/text/original/epub/OEBPS/document_1/document_1.html#_Toc166157923"^^xsd:anyURI ;
    dcat:theme legcons:Division .

F2021L00319:107 a legcons:Division,
        owl:Class,
        dcat:Resource ;
    rdfs:label "Division - D107 Division 4 Variation of approved arrangement"@en-AU ;
    dct:hasPart F2021L00319:108,
        F2021L00319:109 ;
    dct:isPartOf F2021L00319:92 ;
    dct:isReferencedBy F2021L00319: ;
    rdfs:comment "Division 4 Variation of approved arrangement - Abrievated Graph Key: D107"@en-AU ;
    skos:broader F2021L00319:108,
        F2021L00319:109 ;
    skos:definition "Division 4 Variation of approved arrangement"@en-AU ;
    skos:narrower F2021L00319:92 ;
    skos:prefLabel "Division D107"@en-AU ;
    dcat:accessURL <https://www.legislation.gov.au/F2021L00319/2024-04-30/2024-04-30/text/original/epub/OEBPS/document_1/document_1.html#_Toc166157940> ;
    dcat:landingPage "https://www.legislation.gov.au/F2021L00319/2024-04-30/2024-04-30/text/original/epub/OEBPS/document_1/document_1.html#_Toc166157940"^^xsd:anyURI ;
    dcat:theme legcons:Division .

F2021L00319:126 a legcons:Part,
        owl:Class,
        dcat:Resource ;
    rdfs:label "Part - P126 Part 1 Requirements for grant of livestock export licence"@en-AU ;
    dct:hasPart F2021L00319:127,
        F2021L00319:129 ;
    dct:isPartOf F2021L00319:125 ;
    dct:isReferencedBy F2021L00319: ;
    rdfs:comment "Part 1 Requirements for grant of livestock export licence - Abrievated Graph Key: P126"@en-AU ;
    skos:broader F2021L00319:127,
        F2021L00319:129 ;
    skos:definition "Part 1 Requirements for grant of livestock export licence"@en-AU ;
    skos:narrower F2021L00319:125 ;
    skos:prefLabel "Part P126"@en-AU ;
    dcat:accessURL <https://www.legislation.gov.au/F2021L00319/2024-04-30/2024-04-30/text/original/epub/OEBPS/document_1/document_1.html#_Toc166157959> ;
    dcat:landingPage "https://www.legislation.gov.au/F2021L00319/2024-04-30/2024-04-30/text/original/epub/OEBPS/document_1/document_1.html#_Toc166157959"^^xsd:anyURI ;
    dcat:theme legcons:Part .

F2021L00319:129 a legcons:Division,
        owl:Class,
        dcat:Resource ;
    rdfs:label "Division - D129 Division 2 Other matters relating to livestock export licences"@en-AU ;
    dct:hasPart F2021L00319:130,
        F2021L00319:131 ;
    dct:isPartOf F2021L00319:126 ;
    dct:isReferencedBy F2021L00319: ;
    rdfs:comment "Division 2 Other matters relating to livestock export licences - Abrievated Graph Key: D129"@en-AU ;
    skos:broader F2021L00319:130,
        F2021L00319:131 ;
    skos:definition "Division 2 Other matters relating to livestock export licences"@en-AU ;
    skos:narrower F2021L00319:126 ;
    skos:prefLabel "Division D129"@en-AU ;
    dcat:accessURL <https://www.legislation.gov.au/F2021L00319/2024-04-30/2024-04-30/text/original/epub/OEBPS/document_1/document_1.html#_Toc166157962> ;
    dcat:landingPage "https://www.legislation.gov.au/F2021L00319/2024-04-30/2024-04-30/text/original/epub/OEBPS/document_1/document_1.html#_Toc166157962"^^xsd:anyURI ;
    dcat:theme legcons:Division .

F2021L00319:141 a legcons:Division,
        owl:Class,
        dcat:Resource ;
    rdfs:label "Division - D141 Division 3 Exports of cattle to the Republic of Korea"@en-AU ;
    dct:hasPart F2021L00319:142,
        F2021L00319:143 ;
    dct:isPartOf F2021L00319:132 ;
    dct:isReferencedBy F2021L00319: ;
    rdfs:comment "Division 3 Exports of cattle to the Republic of Korea - Abrievated Graph Key: D141"@en-AU ;
    skos:broader F2021L00319:142,
        F2021L00319:143 ;
    skos:definition "Division 3 Exports of cattle to the Republic of Korea"@en-AU ;
    skos:narrower F2021L00319:132 ;
    skos:prefLabel "Division D141"@en-AU ;
    dcat:accessURL <https://www.legislation.gov.au/F2021L00319/2024-04-30/2024-04-30/text/original/epub/OEBPS/document_1/document_1.html#_Toc166157974> ;
    dcat:landingPage "https://www.legislation.gov.au/F2021L00319/2024-04-30/2024-04-30/text/original/epub/OEBPS/document_1/document_1.html#_Toc166157974"^^xsd:anyURI ;
    dcat:theme legcons:Division .

F2021L00319:193 a legcons:Division,
        owl:Class,
        dcat:Resource ;
    rdfs:label "Division - D193 Division 3 Revocation of approved ESCAS"@en-AU ;
    dct:hasPart F2021L00319:194,
        F2021L00319:195 ;
    dct:isPartOf F2021L00319:125 ;
    dct:isReferencedBy F2021L00319: ;
    rdfs:comment "Division 3 Revocation of approved ESCAS - Abrievated Graph Key: D193"@en-AU ;
    skos:broader F2021L00319:194,
        F2021L00319:195 ;
    skos:definition "Division 3 Revocation of approved ESCAS"@en-AU ;
    skos:narrower F2021L00319:125 ;
    skos:prefLabel "Division D193"@en-AU ;
    dcat:accessURL <https://www.legislation.gov.au/F2021L00319/2024-04-30/2024-04-30/text/original/epub/OEBPS/document_1/document_1.html#_Toc166158026> ;
    dcat:landingPage "https://www.legislation.gov.au/F2021L00319/2024-04-30/2024-04-30/text/original/epub/OEBPS/document_1/document_1.html#_Toc166158026"^^xsd:anyURI ;
    dcat:theme legcons:Division .

F2021L00319:200 a legcons:Chapter,
        owl:Class,
        dcat:Resource ;
    rdfs:label "Chapter - C200 Chapter 7 Export permits"@en-AU ;
    dct:hasPart F2021L00319:201,
        F2021L00319:206,
        F2021L00319:211 ;
    dct:isReferencedBy F2021L00319: ;
    rdfs:comment "Chapter 7 Export permits - Abrievated Graph Key: C200"@en-AU ;
    skos:broader F2021L00319:201,
        F2021L00319:206,
        F2021L00319:211 ;
    skos:definition "Chapter 7 Export permits"@en-AU ;
    skos:prefLabel "Chapter C200"@en-AU ;
    dcat:accessURL <https://www.legislation.gov.au/F2021L00319/2024-04-30/2024-04-30/text/original/epub/OEBPS/document_1/document_1.html#_Toc166158033> ;
    dcat:landingPage "https://www.legislation.gov.au/F2021L00319/2024-04-30/2024-04-30/text/original/epub/OEBPS/document_1/document_1.html#_Toc166158033"^^xsd:anyURI ;
    dcat:theme legcons:Chapter .

F2021L00319:216 a legcons:Part,
        owl:Class,
        dcat:Resource ;
    rdfs:label "Part - P216 Part 1 Notices of intention to export"@en-AU ;
    dct:hasPart F2021L00319:217,
        F2021L00319:222 ;
    dct:isPartOf F2021L00319:215 ;
    dct:isReferencedBy F2021L00319: ;
    rdfs:comment "Part 1 Notices of intention to export - Abrievated Graph Key: P216"@en-AU ;
    skos:broader F2021L00319:217,
        F2021L00319:222 ;
    skos:definition "Part 1 Notices of intention to export"@en-AU ;
    skos:narrower F2021L00319:215 ;
    skos:prefLabel "Part P216"@en-AU ;
    dcat:accessURL <https://www.legislation.gov.au/F2021L00319/2024-04-30/2024-04-30/text/original/epub/OEBPS/document_1/document_1.html#_Toc166158049> ;
    dcat:landingPage "https://www.legislation.gov.au/F2021L00319/2024-04-30/2024-04-30/text/original/epub/OEBPS/document_1/document_1.html#_Toc166158049"^^xsd:anyURI ;
    dcat:theme legcons:Part .

F2021L00319:222 a legcons:Division,
        owl:Class,
        dcat:Resource ;
    rdfs:label "Division - D222 Division 2 Approval of notice of intention to export consignment"@en-AU ;
    dct:hasPart F2021L00319:223,
        F2021L00319:229 ;
    dct:isPartOf F2021L00319:216 ;
    dct:isReferencedBy F2021L00319: ;
    rdfs:comment "Division 2 Approval of notice of intention to export consignment - Abrievated Graph Key: D222"@en-AU ;
    skos:broader F2021L00319:223,
        F2021L00319:229 ;
    skos:definition "Division 2 Approval of notice of intention to export consignment"@en-AU ;
    skos:narrower F2021L00319:216 ;
    skos:prefLabel "Division D222"@en-AU ;
    dcat:accessURL <https://www.legislation.gov.au/F2021L00319/2024-04-30/2024-04-30/text/original/epub/OEBPS/document_1/document_1.html#_Toc166158055> ;
    dcat:landingPage "https://www.legislation.gov.au/F2021L00319/2024-04-30/2024-04-30/text/original/epub/OEBPS/document_1/document_1.html#_Toc166158055"^^xsd:anyURI ;
    dcat:theme legcons:Division .

F2021L00319:263 a legcons:Part,
        owl:Class,
        dcat:Resource ;
    rdfs:label "Part - P263 Part 1 Audits"@en-AU ;
    dct:hasPart F2021L00319:264,
        F2021L00319:266 ;
    dct:isPartOf F2021L00319:262 ;
    dct:isReferencedBy F2021L00319: ;
    rdfs:comment "Part 1 Audits - Abrievated Graph Key: P263"@en-AU ;
    skos:broader F2021L00319:264,
        F2021L00319:266 ;
    skos:definition "Part 1 Audits"@en-AU ;
    skos:narrower F2021L00319:262 ;
    skos:prefLabel "Part P263"@en-AU ;
    dcat:accessURL <https://www.legislation.gov.au/F2021L00319/2024-04-30/2024-04-30/text/original/epub/OEBPS/document_1/document_1.html#_Toc166158096> ;
    dcat:landingPage "https://www.legislation.gov.au/F2021L00319/2024-04-30/2024-04-30/text/original/epub/OEBPS/document_1/document_1.html#_Toc166158096"^^xsd:anyURI ;
    dcat:theme legcons:Part .

F2021L00319:271 a legcons:Part,
        owl:Class,
        dcat:Resource ;
    rdfs:label "Part - P271 Part 2 Assessments"@en-AU ;
    dct:hasPart F2021L00319:272,
        F2021L00319:274 ;
    dct:isPartOf F2021L00319:262 ;
    dct:isReferencedBy F2021L00319: ;
    rdfs:comment "Part 2 Assessments - Abrievated Graph Key: P271"@en-AU ;
    skos:broader F2021L00319:272,
        F2021L00319:274 ;
    skos:definition "Part 2 Assessments"@en-AU ;
    skos:narrower F2021L00319:262 ;
    skos:prefLabel "Part P271"@en-AU ;
    dcat:accessURL <https://www.legislation.gov.au/F2021L00319/2024-04-30/2024-04-30/text/original/epub/OEBPS/document_1/document_1.html#_Toc166158104> ;
    dcat:landingPage "https://www.legislation.gov.au/F2021L00319/2024-04-30/2024-04-30/text/original/epub/OEBPS/document_1/document_1.html#_Toc166158104"^^xsd:anyURI ;
    dcat:theme legcons:Part .

F2021L00319:274 a legcons:Division,
        owl:Class,
        dcat:Resource ;
    rdfs:label "Division - D274 Division 2 Carrying out assessments"@en-AU ;
    dct:hasPart F2021L00319:275,
        F2021L00319:276 ;
    dct:isPartOf F2021L00319:271 ;
    dct:isReferencedBy F2021L00319: ;
    rdfs:comment "Division 2 Carrying out assessments - Abrievated Graph Key: D274"@en-AU ;
    skos:broader F2021L00319:275,
        F2021L00319:276 ;
    skos:definition "Division 2 Carrying out assessments"@en-AU ;
    skos:narrower F2021L00319:271 ;
    skos:prefLabel "Division D274"@en-AU ;
    dcat:accessURL <https://www.legislation.gov.au/F2021L00319/2024-04-30/2024-04-30/text/original/epub/OEBPS/document_1/document_1.html#_Toc166158107> ;
    dcat:landingPage "https://www.legislation.gov.au/F2021L00319/2024-04-30/2024-04-30/text/original/epub/OEBPS/document_1/document_1.html#_Toc166158107"^^xsd:anyURI ;
    dcat:theme legcons:Division .

F2021L00319:287 a legcons:Division,
        owl:Class,
        dcat:Resource ;
    rdfs:label "Division - D287 Division 3 Renewal of accreditation"@en-AU ;
    dct:hasPart F2021L00319:288,
        F2021L00319:289 ;
    dct:isPartOf F2021L00319:277 ;
    dct:isReferencedBy F2021L00319: ;
    rdfs:comment "Division 3 Renewal of accreditation - Abrievated Graph Key: D287"@en-AU ;
    skos:broader F2021L00319:288,
        F2021L00319:289 ;
    skos:definition "Division 3 Renewal of accreditation"@en-AU ;
    skos:narrower F2021L00319:277 ;
    skos:prefLabel "Division D287"@en-AU ;
    dcat:accessURL <https://www.legislation.gov.au/F2021L00319/2024-04-30/2024-04-30/text/original/epub/OEBPS/document_1/document_1.html#_Toc166158120> ;
    dcat:landingPage "https://www.legislation.gov.au/F2021L00319/2024-04-30/2024-04-30/text/original/epub/OEBPS/document_1/document_1.html#_Toc166158120"^^xsd:anyURI ;
    dcat:theme legcons:Division .

F2021L00319:290 a legcons:Division,
        owl:Class,
        dcat:Resource ;
    rdfs:label "Division - D290 Division 4 Variation of accreditation"@en-AU ;
    dct:hasPart F2021L00319:291,
        F2021L00319:292 ;
    dct:isPartOf F2021L00319:277 ;
    dct:isReferencedBy F2021L00319: ;
    rdfs:comment "Division 4 Variation of accreditation - Abrievated Graph Key: D290"@en-AU ;
    skos:broader F2021L00319:291,
        F2021L00319:292 ;
    skos:definition "Division 4 Variation of accreditation"@en-AU ;
    skos:narrower F2021L00319:277 ;
    skos:prefLabel "Division D290"@en-AU ;
    dcat:accessURL <https://www.legislation.gov.au/F2021L00319/2024-04-30/2024-04-30/text/original/epub/OEBPS/document_1/document_1.html#_Toc166158123> ;
    dcat:landingPage "https://www.legislation.gov.au/F2021L00319/2024-04-30/2024-04-30/text/original/epub/OEBPS/document_1/document_1.html#_Toc166158123"^^xsd:anyURI ;
    dcat:theme legcons:Division .

F2021L00319:298 a legcons:Division,
        owl:Class,
        dcat:Resource ;
    rdfs:label "Division - D298 Division 6 Revocation of accreditation"@en-AU ;
    dct:hasPart F2021L00319:299,
        F2021L00319:300 ;
    dct:isPartOf F2021L00319:277 ;
    dct:isReferencedBy F2021L00319: ;
    rdfs:comment "Division 6 Revocation of accreditation - Abrievated Graph Key: D298"@en-AU ;
    skos:broader F2021L00319:299,
        F2021L00319:300 ;
    skos:definition "Division 6 Revocation of accreditation"@en-AU ;
    skos:narrower F2021L00319:277 ;
    skos:prefLabel "Division D298"@en-AU ;
    dcat:accessURL <https://www.legislation.gov.au/F2021L00319/2024-04-30/2024-04-30/text/original/epub/OEBPS/document_1/document_1.html#_Toc166158131> ;
    dcat:landingPage "https://www.legislation.gov.au/F2021L00319/2024-04-30/2024-04-30/text/original/epub/OEBPS/document_1/document_1.html#_Toc166158131"^^xsd:anyURI ;
    dcat:theme legcons:Division .

F2021L00319:301 a legcons:Division,
        owl:Class,
        dcat:Resource ;
    rdfs:label "Division - D301 Division 7 Records and reports"@en-AU ;
    dct:hasPart F2021L00319:302,
        F2021L00319:303 ;
    dct:isPartOf F2021L00319:277 ;
    dct:isReferencedBy F2021L00319: ;
    rdfs:comment "Division 7 Records and reports - Abrievated Graph Key: D301"@en-AU ;
    skos:broader F2021L00319:302,
        F2021L00319:303 ;
    skos:definition "Division 7 Records and reports"@en-AU ;
    skos:narrower F2021L00319:277 ;
    skos:prefLabel "Division D301"@en-AU ;
    dcat:accessURL <https://www.legislation.gov.au/F2021L00319/2024-04-30/2024-04-30/text/original/epub/OEBPS/document_1/document_1.html#_Toc166158134> ;
    dcat:landingPage "https://www.legislation.gov.au/F2021L00319/2024-04-30/2024-04-30/text/original/epub/OEBPS/document_1/document_1.html#_Toc166158134"^^xsd:anyURI ;
    dcat:theme legcons:Division .

F2021L00319:326 a legcons:Subdivision,
        owl:Class,
        dcat:Resource ;
    rdfs:label "Subdivision - S326 Subdivision DRevocation of approved export program"@en-AU ;
    dct:hasPart F2021L00319:327,
        F2021L00319:328 ;
    dct:isPartOf F2021L00319:313 ;
    dct:isReferencedBy F2021L00319: ;
    rdfs:comment "Subdivision DRevocation of approved export program - Abrievated Graph Key: S326"@en-AU ;
    skos:broader F2021L00319:327,
        F2021L00319:328 ;
    skos:definition "Subdivision DRevocation of approved export program"@en-AU ;
    skos:narrower F2021L00319:313 ;
    skos:prefLabel "Subdivision S326"@en-AU ;
    dcat:accessURL <https://www.legislation.gov.au/F2021L00319/2024-04-30/2024-04-30/text/original/epub/OEBPS/document_1/document_1.html#_Toc166158159> ;
    dcat:landingPage "https://www.legislation.gov.au/F2021L00319/2024-04-30/2024-04-30/text/original/epub/OEBPS/document_1/document_1.html#_Toc166158159"^^xsd:anyURI ;
    dcat:theme legcons:Subdivision .

F2021L00319:335 a legcons:Division,
        owl:Class,
        dcat:Resource ;
    rdfs:label "Division - D335 Division 4 Other powers of Secretary"@en-AU ;
    dct:hasPart F2021L00319:336,
        F2021L00319:337 ;
    dct:isPartOf F2021L00319:310 ;
    dct:isReferencedBy F2021L00319: ;
    rdfs:comment "Division 4 Other powers of Secretary - Abrievated Graph Key: D335"@en-AU ;
    skos:broader F2021L00319:336,
        F2021L00319:337 ;
    skos:definition "Division 4 Other powers of Secretary"@en-AU ;
    skos:narrower F2021L00319:310 ;
    skos:prefLabel "Division D335"@en-AU ;
    dcat:accessURL <https://www.legislation.gov.au/F2021L00319/2024-04-30/2024-04-30/text/original/epub/OEBPS/document_1/document_1.html#_Toc166158168> ;
    dcat:landingPage "https://www.legislation.gov.au/F2021L00319/2024-04-30/2024-04-30/text/original/epub/OEBPS/document_1/document_1.html#_Toc166158168"^^xsd:anyURI ;
    dcat:theme legcons:Division .

F2021L00319:338 a legcons:Division,
        owl:Class,
        dcat:Resource ;
    rdfs:label "Division - D338 Division 5 Other provisions"@en-AU ;
    dct:hasPart F2021L00319:339,
        F2021L00319:340 ;
    dct:isPartOf F2021L00319:310 ;
    dct:isReferencedBy F2021L00319: ;
    rdfs:comment "Division 5 Other provisions - Abrievated Graph Key: D338"@en-AU ;
    skos:broader F2021L00319:339,
        F2021L00319:340 ;
    skos:definition "Division 5 Other provisions"@en-AU ;
    skos:narrower F2021L00319:310 ;
    skos:prefLabel "Division D338"@en-AU ;
    dcat:accessURL <https://www.legislation.gov.au/F2021L00319/2024-04-30/2024-04-30/text/original/epub/OEBPS/document_1/document_1.html#_Toc166158171> ;
    dcat:landingPage "https://www.legislation.gov.au/F2021L00319/2024-04-30/2024-04-30/text/original/epub/OEBPS/document_1/document_1.html#_Toc166158171"^^xsd:anyURI ;
    dcat:theme legcons:Division .

F2021L00319:341 a legcons:Part,
        owl:Class,
        dcat:Resource ;
    rdfs:label "Part - P341 Part 5 Powers of the Secretary"@en-AU ;
    dct:hasPart F2021L00319:342,
        F2021L00319:343 ;
    dct:isPartOf F2021L00319:262 ;
    dct:isReferencedBy F2021L00319: ;
    rdfs:comment "Part 5 Powers of the Secretary - Abrievated Graph Key: P341"@en-AU ;
    skos:broader F2021L00319:342,
        F2021L00319:343 ;
    skos:definition "Part 5 Powers of the Secretary"@en-AU ;
    skos:narrower F2021L00319:262 ;
    skos:prefLabel "Part P341"@en-AU ;
    dcat:accessURL <https://www.legislation.gov.au/F2021L00319/2024-04-30/2024-04-30/text/original/epub/OEBPS/document_1/document_1.html#_Toc166158174> ;
    dcat:landingPage "https://www.legislation.gov.au/F2021L00319/2024-04-30/2024-04-30/text/original/epub/OEBPS/document_1/document_1.html#_Toc166158174"^^xsd:anyURI ;
    dcat:theme legcons:Part .

F2021L00319:344 a legcons:Part,
        owl:Class,
        dcat:Resource ;
    rdfs:label "Part - P344 Part 6 Functions and powers of authorised officers"@en-AU ;
    dct:hasPart F2021L00319:345,
        F2021L00319:346 ;
    dct:isPartOf F2021L00319:262 ;
    dct:isReferencedBy F2021L00319: ;
    rdfs:comment "Part 6 Functions and powers of authorised officers - Abrievated Graph Key: P344"@en-AU ;
    skos:broader F2021L00319:345,
        F2021L00319:346 ;
    skos:definition "Part 6 Functions and powers of authorised officers"@en-AU ;
    skos:narrower F2021L00319:262 ;
    skos:prefLabel "Part P344"@en-AU ;
    dcat:accessURL <https://www.legislation.gov.au/F2021L00319/2024-04-30/2024-04-30/text/original/epub/OEBPS/document_1/document_1.html#_Toc166158177> ;
    dcat:landingPage "https://www.legislation.gov.au/F2021L00319/2024-04-30/2024-04-30/text/original/epub/OEBPS/document_1/document_1.html#_Toc166158177"^^xsd:anyURI ;
    dcat:theme legcons:Part .

F2021L00319:366 a legcons:Part,
        owl:Class,
        dcat:Resource ;
    rdfs:label "Part - P366 Part 4 Damaged or destroyed prescribed livestock prescribed live animals or prescribed animal reproductive material"@en-AU ;
    dct:hasPart F2021L00319:367,
        F2021L00319:368 ;
    dct:isPartOf F2021L00319:350 ;
    dct:isReferencedBy F2021L00319: ;
    rdfs:comment "Part 4 Damaged or destroyed prescribed livestock prescribed live animals or prescribed animal reproductive material - Abrievated Graph Key: P366"@en-AU ;
    skos:broader F2021L00319:367,
        F2021L00319:368 ;
    skos:definition "Part 4 Damaged or destroyed prescribed livestock prescribed live animals or prescribed animal reproductive material"@en-AU ;
    skos:narrower F2021L00319:350 ;
    skos:prefLabel "Part P366"@en-AU ;
    dcat:accessURL <https://www.legislation.gov.au/F2021L00319/2024-04-30/2024-04-30/text/original/epub/OEBPS/document_1/document_1.html#_Toc166158199> ;
    dcat:landingPage "https://www.legislation.gov.au/F2021L00319/2024-04-30/2024-04-30/text/original/epub/OEBPS/document_1/document_1.html#_Toc166158199"^^xsd:anyURI ;
    dcat:theme legcons:Part .

F2021L00319:376 a legcons:Part,
        owl:Class,
        dcat:Resource ;
    rdfs:label "Part - P376 Part 2 Registered establishments"@en-AU ;
    dct:hasPart F2021L00319:377,
        F2021L00319:378 ;
    dct:isPartOf F2021L00319:373 ;
    dct:isReferencedBy F2021L00319: ;
    rdfs:comment "Part 2 Registered establishments - Abrievated Graph Key: P376"@en-AU ;
    skos:broader F2021L00319:377,
        F2021L00319:378 ;
    skos:definition "Part 2 Registered establishments"@en-AU ;
    skos:narrower F2021L00319:373 ;
    skos:prefLabel "Part P376"@en-AU ;
    dcat:accessURL <https://www.legislation.gov.au/F2021L00319/2024-04-30/2024-04-30/text/original/epub/OEBPS/document_1/document_1.html#_Toc166158209> ;
    dcat:landingPage "https://www.legislation.gov.au/F2021L00319/2024-04-30/2024-04-30/text/original/epub/OEBPS/document_1/document_1.html#_Toc166158209"^^xsd:anyURI ;
    dcat:theme legcons:Part .

F2021L00319:393 a legcons:Division,
        owl:Class,
        dcat:Resource ;
    rdfs:label "Division - D393 Division 3 Official marking devices"@en-AU ;
    dct:hasPart F2021L00319:394,
        F2021L00319:395 ;
    dct:isPartOf F2021L00319:383 ;
    dct:isReferencedBy F2021L00319: ;
    rdfs:comment "Division 3 Official marking devices - Abrievated Graph Key: D393"@en-AU ;
    skos:broader F2021L00319:394,
        F2021L00319:395 ;
    skos:definition "Division 3 Official marking devices"@en-AU ;
    skos:narrower F2021L00319:383 ;
    skos:prefLabel "Division D393"@en-AU ;
    dcat:accessURL <https://www.legislation.gov.au/F2021L00319/2024-04-30/2024-04-30/text/original/epub/OEBPS/document_1/document_1.html#_Toc166158226> ;
    dcat:landingPage "https://www.legislation.gov.au/F2021L00319/2024-04-30/2024-04-30/text/original/epub/OEBPS/document_1/document_1.html#_Toc166158226"^^xsd:anyURI ;
    dcat:theme legcons:Division .

F2021L00319:396 a legcons:Part,
        owl:Class,
        dcat:Resource ;
    rdfs:label "Part - P396 Part 5 Powers and officials"@en-AU ;
    dct:hasPart F2021L00319:397,
        F2021L00319:405 ;
    dct:isPartOf F2021L00319:373 ;
    dct:isReferencedBy F2021L00319: ;
    rdfs:comment "Part 5 Powers and officials - Abrievated Graph Key: P396"@en-AU ;
    skos:broader F2021L00319:397,
        F2021L00319:405 ;
    skos:definition "Part 5 Powers and officials"@en-AU ;
    skos:narrower F2021L00319:373 ;
    skos:prefLabel "Part P396"@en-AU ;
    dcat:accessURL <https://www.legislation.gov.au/F2021L00319/2024-04-30/2024-04-30/text/original/epub/OEBPS/document_1/document_1.html#_Toc166158229> ;
    dcat:landingPage "https://www.legislation.gov.au/F2021L00319/2024-04-30/2024-04-30/text/original/epub/OEBPS/document_1/document_1.html#_Toc166158229"^^xsd:anyURI ;
    dcat:theme legcons:Part .

F2021L00319:40 a legcons:Division,
        owl:Class,
        dcat:Resource ;
    rdfs:label "Division - D40 Division 3 Prescribed live animals"@en-AU ;
    dct:hasPart F2021L00319:41,
        F2021L00319:42 ;
    dct:isPartOf F2021L00319:9 ;
    dct:isReferencedBy F2021L00319: ;
    rdfs:comment "Division 3 Prescribed live animals - Abrievated Graph Key: D40"@en-AU ;
    skos:broader F2021L00319:41,
        F2021L00319:42 ;
    skos:definition "Division 3 Prescribed live animals"@en-AU ;
    skos:narrower F2021L00319:9 ;
    skos:prefLabel "Division D40"@en-AU ;
    dcat:accessURL <https://www.legislation.gov.au/F2021L00319/2024-04-30/2024-04-30/text/original/epub/OEBPS/document_1/document_1.html#_Toc166157873> ;
    dcat:landingPage "https://www.legislation.gov.au/F2021L00319/2024-04-30/2024-04-30/text/original/epub/OEBPS/document_1/document_1.html#_Toc166157873"^^xsd:anyURI ;
    dcat:theme legcons:Division .

F2021L00319:405 a legcons:Division,
        owl:Class,
        dcat:Resource ;
    rdfs:label "Division - D405 Division 2 Approved export programs"@en-AU ;
    dct:hasPart F2021L00319:406,
        F2021L00319:414 ;
    dct:isPartOf F2021L00319:396 ;
    dct:isReferencedBy F2021L00319: ;
    rdfs:comment "Division 2 Approved export programs - Abrievated Graph Key: D405"@en-AU ;
    skos:broader F2021L00319:406,
        F2021L00319:414 ;
    skos:definition "Division 2 Approved export programs"@en-AU ;
    skos:narrower F2021L00319:396 ;
    skos:prefLabel "Division D405"@en-AU ;
    dcat:accessURL <https://www.legislation.gov.au/F2021L00319/2024-04-30/2024-04-30/text/original/epub/OEBPS/document_1/document_1.html#_Toc166158238> ;
    dcat:landingPage "https://www.legislation.gov.au/F2021L00319/2024-04-30/2024-04-30/text/original/epub/OEBPS/document_1/document_1.html#_Toc166158238"^^xsd:anyURI ;
    dcat:theme legcons:Division .

F2021L00319:414 a legcons:Subdivision,
        owl:Class,
        dcat:Resource ;
    rdfs:label "Subdivision - S414 Subdivision BSecretarys approved export programs"@en-AU ;
    dct:hasPart F2021L00319:415,
        F2021L00319:416 ;
    dct:isPartOf F2021L00319:405 ;
    dct:isReferencedBy F2021L00319: ;
    rdfs:comment "Subdivision BSecretarys approved export programs - Abrievated Graph Key: S414"@en-AU ;
    skos:broader F2021L00319:415,
        F2021L00319:416 ;
    skos:definition "Subdivision BSecretarys approved export programs"@en-AU ;
    skos:narrower F2021L00319:405 ;
    skos:prefLabel "Subdivision S414"@en-AU ;
    dcat:accessURL <https://www.legislation.gov.au/F2021L00319/2024-04-30/2024-04-30/text/original/epub/OEBPS/document_1/document_1.html#_Toc166158247> ;
    dcat:landingPage "https://www.legislation.gov.au/F2021L00319/2024-04-30/2024-04-30/text/original/epub/OEBPS/document_1/document_1.html#_Toc166158247"^^xsd:anyURI ;
    dcat:theme legcons:Subdivision .

F2021L00319:46 a legcons:Part,
        owl:Class,
        dcat:Resource ;
    rdfs:label "Part - P46 Part 2 Requirements for registration and other matters"@en-AU ;
    dct:hasPart F2021L00319:47,
        F2021L00319:50 ;
    dct:isPartOf F2021L00319:43 ;
    dct:isReferencedBy F2021L00319: ;
    rdfs:comment "Part 2 Requirements for registration and other matters - Abrievated Graph Key: P46"@en-AU ;
    skos:broader F2021L00319:47,
        F2021L00319:50 ;
    skos:definition "Part 2 Requirements for registration and other matters"@en-AU ;
    skos:narrower F2021L00319:43 ;
    skos:prefLabel "Part P46"@en-AU ;
    dcat:accessURL <https://www.legislation.gov.au/F2021L00319/2024-04-30/2024-04-30/text/original/epub/OEBPS/document_1/document_1.html#_Toc166157879> ;
    dcat:landingPage "https://www.legislation.gov.au/F2021L00319/2024-04-30/2024-04-30/text/original/epub/OEBPS/document_1/document_1.html#_Toc166157879"^^xsd:anyURI ;
    dcat:theme legcons:Part .

F2021L00319:47 a legcons:Division,
        owl:Class,
        dcat:Resource ;
    rdfs:label "Division - D47 Division 1 Requirements for registration"@en-AU ;
    dct:hasPart F2021L00319:48,
        F2021L00319:49 ;
    dct:isPartOf F2021L00319:46 ;
    dct:isReferencedBy F2021L00319: ;
    rdfs:comment "Division 1 Requirements for registration - Abrievated Graph Key: D47"@en-AU ;
    skos:broader F2021L00319:48,
        F2021L00319:49 ;
    skos:definition "Division 1 Requirements for registration"@en-AU ;
    skos:narrower F2021L00319:46 ;
    skos:prefLabel "Division D47"@en-AU ;
    dcat:accessURL <https://www.legislation.gov.au/F2021L00319/2024-04-30/2024-04-30/text/original/epub/OEBPS/document_1/document_1.html#_Toc166157880> ;
    dcat:landingPage "https://www.legislation.gov.au/F2021L00319/2024-04-30/2024-04-30/text/original/epub/OEBPS/document_1/document_1.html#_Toc166157880"^^xsd:anyURI ;
    dcat:theme legcons:Division .

F2021L00319:59 a legcons:Part,
        owl:Class,
        dcat:Resource ;
    rdfs:label "Part - P59 Part 4 Renewal of registration"@en-AU ;
    dct:hasPart F2021L00319:60,
        F2021L00319:61 ;
    dct:isPartOf F2021L00319:43 ;
    dct:isReferencedBy F2021L00319: ;
    rdfs:comment "Part 4 Renewal of registration - Abrievated Graph Key: P59"@en-AU ;
    skos:broader F2021L00319:60,
        F2021L00319:61 ;
    skos:definition "Part 4 Renewal of registration"@en-AU ;
    skos:narrower F2021L00319:43 ;
    skos:prefLabel "Part P59"@en-AU ;
    dcat:accessURL <https://www.legislation.gov.au/F2021L00319/2024-04-30/2024-04-30/text/original/epub/OEBPS/document_1/document_1.html#_Toc166157892> ;
    dcat:landingPage "https://www.legislation.gov.au/F2021L00319/2024-04-30/2024-04-30/text/original/epub/OEBPS/document_1/document_1.html#_Toc166157892"^^xsd:anyURI ;
    dcat:theme legcons:Part .

F2021L00319:74 a legcons:Chapter,
        owl:Class,
        dcat:Resource ;
    rdfs:label "Chapter - C74 Chapter 5 Approved arrangements"@en-AU ;
    dct:hasPart F2021L00319:120,
        F2021L00319:75,
        F2021L00319:92 ;
    dct:isReferencedBy F2021L00319: ;
    rdfs:comment "Chapter 5 Approved arrangements - Abrievated Graph Key: C74"@en-AU ;
    skos:broader F2021L00319:120,
        F2021L00319:75,
        F2021L00319:92 ;
    skos:definition "Chapter 5 Approved arrangements"@en-AU ;
    skos:prefLabel "Chapter C74"@en-AU ;
    dcat:accessURL <https://www.legislation.gov.au/F2021L00319/2024-04-30/2024-04-30/text/original/epub/OEBPS/document_1/document_1.html#_Toc166157907> ;
    dcat:landingPage "https://www.legislation.gov.au/F2021L00319/2024-04-30/2024-04-30/text/original/epub/OEBPS/document_1/document_1.html#_Toc166157907"^^xsd:anyURI ;
    dcat:theme legcons:Chapter .

F2021L00319:110 a legcons:Division,
        owl:Class,
        dcat:Resource ;
    rdfs:label "Division - D110 Division 5 Suspension of approved arrangement"@en-AU ;
    dct:hasPart F2021L00319:111,
        F2021L00319:112,
        F2021L00319:113 ;
    dct:isPartOf F2021L00319:92 ;
    dct:isReferencedBy F2021L00319: ;
    rdfs:comment "Division 5 Suspension of approved arrangement - Abrievated Graph Key: D110"@en-AU ;
    skos:broader F2021L00319:111,
        F2021L00319:112,
        F2021L00319:113 ;
    skos:definition "Division 5 Suspension of approved arrangement"@en-AU ;
    skos:narrower F2021L00319:92 ;
    skos:prefLabel "Division D110"@en-AU ;
    dcat:accessURL <https://www.legislation.gov.au/F2021L00319/2024-04-30/2024-04-30/text/original/epub/OEBPS/document_1/document_1.html#_Toc166157943> ;
    dcat:landingPage "https://www.legislation.gov.au/F2021L00319/2024-04-30/2024-04-30/text/original/epub/OEBPS/document_1/document_1.html#_Toc166157943"^^xsd:anyURI ;
    dcat:theme legcons:Division .

F2021L00319:189 a legcons:Division,
        owl:Class,
        dcat:Resource ;
    rdfs:label "Division - D189 Division 2 Variation of approved ESCAS"@en-AU ;
    dct:hasPart F2021L00319:190,
        F2021L00319:191,
        F2021L00319:192 ;
    dct:isPartOf F2021L00319:125 ;
    dct:isReferencedBy F2021L00319: ;
    rdfs:comment "Division 2 Variation of approved ESCAS - Abrievated Graph Key: D189"@en-AU ;
    skos:broader F2021L00319:190,
        F2021L00319:191,
        F2021L00319:192 ;
    skos:definition "Division 2 Variation of approved ESCAS"@en-AU ;
    skos:narrower F2021L00319:125 ;
    skos:prefLabel "Division D189"@en-AU ;
    dcat:accessURL <https://www.legislation.gov.au/F2021L00319/2024-04-30/2024-04-30/text/original/epub/OEBPS/document_1/document_1.html#_Toc166158022> ;
    dcat:landingPage "https://www.legislation.gov.au/F2021L00319/2024-04-30/2024-04-30/text/original/epub/OEBPS/document_1/document_1.html#_Toc166158022"^^xsd:anyURI ;
    dcat:theme legcons:Division .

F2021L00319:211 a legcons:Part,
        owl:Class,
        dcat:Resource ;
    rdfs:label "Part - P211 Part 3 Other matters"@en-AU ;
    dct:hasPart F2021L00319:212,
        F2021L00319:213,
        F2021L00319:214 ;
    dct:isPartOf F2021L00319:200 ;
    dct:isReferencedBy F2021L00319: ;
    rdfs:comment "Part 3 Other matters - Abrievated Graph Key: P211"@en-AU ;
    skos:broader F2021L00319:212,
        F2021L00319:213,
        F2021L00319:214 ;
    skos:definition "Part 3 Other matters"@en-AU ;
    skos:narrower F2021L00319:200 ;
    skos:prefLabel "Part P211"@en-AU ;
    dcat:accessURL <https://www.legislation.gov.au/F2021L00319/2024-04-30/2024-04-30/text/original/epub/OEBPS/document_1/document_1.html#_Toc166158044> ;
    dcat:landingPage "https://www.legislation.gov.au/F2021L00319/2024-04-30/2024-04-30/text/original/epub/OEBPS/document_1/document_1.html#_Toc166158044"^^xsd:anyURI ;
    dcat:theme legcons:Part .

F2021L00319:235 a legcons:Part,
        owl:Class,
        dcat:Resource ;
    rdfs:label "Part - P235 Part 2 Official marks"@en-AU ;
    dct:hasPart F2021L00319:236,
        F2021L00319:243,
        F2021L00319:255 ;
    dct:isPartOf F2021L00319:215 ;
    dct:isReferencedBy F2021L00319: ;
    rdfs:comment "Part 2 Official marks - Abrievated Graph Key: P235"@en-AU ;
    skos:broader F2021L00319:236,
        F2021L00319:243,
        F2021L00319:255 ;
    skos:definition "Part 2 Official marks"@en-AU ;
    skos:narrower F2021L00319:215 ;
    skos:prefLabel "Part P235"@en-AU ;
    dcat:accessURL <https://www.legislation.gov.au/F2021L00319/2024-04-30/2024-04-30/text/original/epub/OEBPS/document_1/document_1.html#_Toc166158068> ;
    dcat:landingPage "https://www.legislation.gov.au/F2021L00319/2024-04-30/2024-04-30/text/original/epub/OEBPS/document_1/document_1.html#_Toc166158068"^^xsd:anyURI ;
    dcat:theme legcons:Part .

F2021L00319:306 a legcons:Division,
        owl:Class,
        dcat:Resource ;
    rdfs:label "Division - D306 Division 9 Matters relating to applications"@en-AU ;
    dct:hasPart F2021L00319:307,
        F2021L00319:308,
        F2021L00319:309 ;
    dct:isPartOf F2021L00319:277 ;
    dct:isReferencedBy F2021L00319: ;
    rdfs:comment "Division 9 Matters relating to applications - Abrievated Graph Key: D306"@en-AU ;
    skos:broader F2021L00319:307,
        F2021L00319:308,
        F2021L00319:309 ;
    skos:definition "Division 9 Matters relating to applications"@en-AU ;
    skos:narrower F2021L00319:277 ;
    skos:prefLabel "Division D306"@en-AU ;
    dcat:accessURL <https://www.legislation.gov.au/F2021L00319/2024-04-30/2024-04-30/text/original/epub/OEBPS/document_1/document_1.html#_Toc166158139> ;
    dcat:landingPage "https://www.legislation.gov.au/F2021L00319/2024-04-30/2024-04-30/text/original/epub/OEBPS/document_1/document_1.html#_Toc166158139"^^xsd:anyURI ;
    dcat:theme legcons:Division .

F2021L00319:314 a legcons:Subdivision,
        owl:Class,
        dcat:Resource ;
    rdfs:label "Subdivision - S314 Subdivision AApproval of program of export operations"@en-AU ;
    dct:hasPart F2021L00319:315,
        F2021L00319:316,
        F2021L00319:317 ;
    dct:isPartOf F2021L00319:313 ;
    dct:isReferencedBy F2021L00319: ;
    rdfs:comment "Subdivision AApproval of program of export operations - Abrievated Graph Key: S314"@en-AU ;
    skos:broader F2021L00319:315,
        F2021L00319:316,
        F2021L00319:317 ;
    skos:definition "Subdivision AApproval of program of export operations"@en-AU ;
    skos:narrower F2021L00319:313 ;
    skos:prefLabel "Subdivision S314"@en-AU ;
    dcat:accessURL <https://www.legislation.gov.au/F2021L00319/2024-04-30/2024-04-30/text/original/epub/OEBPS/document_1/document_1.html#_Toc166158147> ;
    dcat:landingPage "https://www.legislation.gov.au/F2021L00319/2024-04-30/2024-04-30/text/original/epub/OEBPS/document_1/document_1.html#_Toc166158147"^^xsd:anyURI ;
    dcat:theme legcons:Subdivision .

F2021L00319:318 a legcons:Subdivision,
        owl:Class,
        dcat:Resource ;
    rdfs:label "Subdivision - S318 Subdivision BVariation of approved export program"@en-AU ;
    dct:hasPart F2021L00319:319,
        F2021L00319:320,
        F2021L00319:321 ;
    dct:isPartOf F2021L00319:313 ;
    dct:isReferencedBy F2021L00319: ;
    rdfs:comment "Subdivision BVariation of approved export program - Abrievated Graph Key: S318"@en-AU ;
    skos:broader F2021L00319:319,
        F2021L00319:320,
        F2021L00319:321 ;
    skos:definition "Subdivision BVariation of approved export program"@en-AU ;
    skos:narrower F2021L00319:313 ;
    skos:prefLabel "Subdivision S318"@en-AU ;
    dcat:accessURL <https://www.legislation.gov.au/F2021L00319/2024-04-30/2024-04-30/text/original/epub/OEBPS/document_1/document_1.html#_Toc166158151> ;
    dcat:landingPage "https://www.legislation.gov.au/F2021L00319/2024-04-30/2024-04-30/text/original/epub/OEBPS/document_1/document_1.html#_Toc166158151"^^xsd:anyURI ;
    dcat:theme legcons:Subdivision .

F2021L00319:322 a legcons:Subdivision,
        owl:Class,
        dcat:Resource ;
    rdfs:label "Subdivision - S322 Subdivision CSuspension of approved export program"@en-AU ;
    dct:hasPart F2021L00319:323,
        F2021L00319:324,
        F2021L00319:325 ;
    dct:isPartOf F2021L00319:313 ;
    dct:isReferencedBy F2021L00319: ;
    rdfs:comment "Subdivision CSuspension of approved export program - Abrievated Graph Key: S322"@en-AU ;
    skos:broader F2021L00319:323,
        F2021L00319:324,
        F2021L00319:325 ;
    skos:definition "Subdivision CSuspension of approved export program"@en-AU ;
    skos:narrower F2021L00319:313 ;
    skos:prefLabel "Subdivision S322"@en-AU ;
    dcat:accessURL <https://www.legislation.gov.au/F2021L00319/2024-04-30/2024-04-30/text/original/epub/OEBPS/document_1/document_1.html#_Toc166158155> ;
    dcat:landingPage "https://www.legislation.gov.au/F2021L00319/2024-04-30/2024-04-30/text/original/epub/OEBPS/document_1/document_1.html#_Toc166158155"^^xsd:anyURI ;
    dcat:theme legcons:Subdivision .

F2021L00319:331 a legcons:Division,
        owl:Class,
        dcat:Resource ;
    rdfs:label "Division - D331 Division 3 Secretarys approved export programs"@en-AU ;
    dct:hasPart F2021L00319:332,
        F2021L00319:333,
        F2021L00319:334 ;
    dct:isPartOf F2021L00319:310 ;
    dct:isReferencedBy F2021L00319: ;
    rdfs:comment "Division 3 Secretarys approved export programs - Abrievated Graph Key: D331"@en-AU ;
    skos:broader F2021L00319:332,
        F2021L00319:333,
        F2021L00319:334 ;
    skos:definition "Division 3 Secretarys approved export programs"@en-AU ;
    skos:narrower F2021L00319:310 ;
    skos:prefLabel "Division D331"@en-AU ;
    dcat:accessURL <https://www.legislation.gov.au/F2021L00319/2024-04-30/2024-04-30/text/original/epub/OEBPS/document_1/document_1.html#_Toc166158164> ;
    dcat:landingPage "https://www.legislation.gov.au/F2021L00319/2024-04-30/2024-04-30/text/original/epub/OEBPS/document_1/document_1.html#_Toc166158164"^^xsd:anyURI ;
    dcat:theme legcons:Division .

F2021L00319:379 a legcons:Part,
        owl:Class,
        dcat:Resource ;
    rdfs:label "Part - P379 Part 3 Livestock export licences exporter supply chain assurance systems"@en-AU ;
    dct:hasPart F2021L00319:380,
        F2021L00319:381,
        F2021L00319:382 ;
    dct:isPartOf F2021L00319:373 ;
    dct:isReferencedBy F2021L00319: ;
    rdfs:comment "Part 3 Livestock export licences exporter supply chain assurance systems - Abrievated Graph Key: P379"@en-AU ;
    skos:broader F2021L00319:380,
        F2021L00319:381,
        F2021L00319:382 ;
    skos:definition "Part 3 Livestock export licences exporter supply chain assurance systems"@en-AU ;
    skos:narrower F2021L00319:373 ;
    skos:prefLabel "Part P379"@en-AU ;
    dcat:accessURL <https://www.legislation.gov.au/F2021L00319/2024-04-30/2024-04-30/text/original/epub/OEBPS/document_1/document_1.html#_Toc166158212> ;
    dcat:landingPage "https://www.legislation.gov.au/F2021L00319/2024-04-30/2024-04-30/text/original/epub/OEBPS/document_1/document_1.html#_Toc166158212"^^xsd:anyURI ;
    dcat:theme legcons:Part .

F2021L00319:383 a legcons:Part,
        owl:Class,
        dcat:Resource ;
    rdfs:label "Part - P383 Part 4 Other matters relating to export"@en-AU ;
    dct:hasPart F2021L00319:384,
        F2021L00319:389,
        F2021L00319:393 ;
    dct:isPartOf F2021L00319:373 ;
    dct:isReferencedBy F2021L00319: ;
    rdfs:comment "Part 4 Other matters relating to export - Abrievated Graph Key: P383"@en-AU ;
    skos:broader F2021L00319:384,
        F2021L00319:389,
        F2021L00319:393 ;
    skos:definition "Part 4 Other matters relating to export"@en-AU ;
    skos:narrower F2021L00319:373 ;
    skos:prefLabel "Part P383"@en-AU ;
    dcat:accessURL <https://www.legislation.gov.au/F2021L00319/2024-04-30/2024-04-30/text/original/epub/OEBPS/document_1/document_1.html#_Toc166158216> ;
    dcat:landingPage "https://www.legislation.gov.au/F2021L00319/2024-04-30/2024-04-30/text/original/epub/OEBPS/document_1/document_1.html#_Toc166158216"^^xsd:anyURI ;
    dcat:theme legcons:Part .

F2021L00319:389 a legcons:Division,
        owl:Class,
        dcat:Resource ;
    rdfs:label "Division - D389 Division 2 Official marks"@en-AU ;
    dct:hasPart F2021L00319:390,
        F2021L00319:391,
        F2021L00319:392 ;
    dct:isPartOf F2021L00319:383 ;
    dct:isReferencedBy F2021L00319: ;
    rdfs:comment "Division 2 Official marks - Abrievated Graph Key: D389"@en-AU ;
    skos:broader F2021L00319:390,
        F2021L00319:391,
        F2021L00319:392 ;
    skos:definition "Division 2 Official marks"@en-AU ;
    skos:narrower F2021L00319:383 ;
    skos:prefLabel "Division D389"@en-AU ;
    dcat:accessURL <https://www.legislation.gov.au/F2021L00319/2024-04-30/2024-04-30/text/original/epub/OEBPS/document_1/document_1.html#_Toc166158222> ;
    dcat:landingPage "https://www.legislation.gov.au/F2021L00319/2024-04-30/2024-04-30/text/original/epub/OEBPS/document_1/document_1.html#_Toc166158222"^^xsd:anyURI ;
    dcat:theme legcons:Division .

F2021L00319:68 a legcons:Part,
        owl:Class,
        dcat:Resource ;
    rdfs:label "Part - P68 Part 8 Matters relating to applications"@en-AU ;
    dct:hasPart F2021L00319:69,
        F2021L00319:70,
        F2021L00319:71 ;
    dct:isPartOf F2021L00319:43 ;
    dct:isReferencedBy F2021L00319: ;
    rdfs:comment "Part 8 Matters relating to applications - Abrievated Graph Key: P68"@en-AU ;
    skos:broader F2021L00319:69,
        F2021L00319:70,
        F2021L00319:71 ;
    skos:definition "Part 8 Matters relating to applications"@en-AU ;
    skos:narrower F2021L00319:43 ;
    skos:prefLabel "Part P68"@en-AU ;
    dcat:accessURL <https://www.legislation.gov.au/F2021L00319/2024-04-30/2024-04-30/text/original/epub/OEBPS/document_1/document_1.html#_Toc166157901> ;
    dcat:landingPage "https://www.legislation.gov.au/F2021L00319/2024-04-30/2024-04-30/text/original/epub/OEBPS/document_1/document_1.html#_Toc166157901"^^xsd:anyURI ;
    dcat:theme legcons:Part .

F2021L00319:120 a legcons:Part,
        owl:Class,
        dcat:Resource ;
    rdfs:label "Part - P120 Part 3 Matters relating to applications"@en-AU ;
    dct:hasPart F2021L00319:121,
        F2021L00319:122,
        F2021L00319:123,
        F2021L00319:124 ;
    dct:isPartOf F2021L00319:74 ;
    dct:isReferencedBy F2021L00319: ;
    rdfs:comment "Part 3 Matters relating to applications - Abrievated Graph Key: P120"@en-AU ;
    skos:broader F2021L00319:121,
        F2021L00319:122,
        F2021L00319:123,
        F2021L00319:124 ;
    skos:definition "Part 3 Matters relating to applications"@en-AU ;
    skos:narrower F2021L00319:74 ;
    skos:prefLabel "Part P120"@en-AU ;
    dcat:accessURL <https://www.legislation.gov.au/F2021L00319/2024-04-30/2024-04-30/text/original/epub/OEBPS/document_1/document_1.html#_Toc166157953> ;
    dcat:landingPage "https://www.legislation.gov.au/F2021L00319/2024-04-30/2024-04-30/text/original/epub/OEBPS/document_1/document_1.html#_Toc166157953"^^xsd:anyURI ;
    dcat:theme legcons:Part .

F2021L00319:201 a legcons:Part,
        owl:Class,
        dcat:Resource ;
    rdfs:label "Part - P201 Part 1 Issue of export permit"@en-AU ;
    dct:hasPart F2021L00319:202,
        F2021L00319:203,
        F2021L00319:204,
        F2021L00319:205 ;
    dct:isPartOf F2021L00319:200 ;
    dct:isReferencedBy F2021L00319: ;
    rdfs:comment "Part 1 Issue of export permit - Abrievated Graph Key: P201"@en-AU ;
    skos:broader F2021L00319:202,
        F2021L00319:203,
        F2021L00319:204,
        F2021L00319:205 ;
    skos:definition "Part 1 Issue of export permit"@en-AU ;
    skos:narrower F2021L00319:200 ;
    skos:prefLabel "Part P201"@en-AU ;
    dcat:accessURL <https://www.legislation.gov.au/F2021L00319/2024-04-30/2024-04-30/text/original/epub/OEBPS/document_1/document_1.html#_Toc166158034> ;
    dcat:landingPage "https://www.legislation.gov.au/F2021L00319/2024-04-30/2024-04-30/text/original/epub/OEBPS/document_1/document_1.html#_Toc166158034"^^xsd:anyURI ;
    dcat:theme legcons:Part .

F2021L00319:206 a legcons:Part,
        owl:Class,
        dcat:Resource ;
    rdfs:label "Part - P206 Part 2 Variation suspension and revocation of export permit"@en-AU ;
    dct:hasPart F2021L00319:207,
        F2021L00319:208,
        F2021L00319:209,
        F2021L00319:210 ;
    dct:isPartOf F2021L00319:200 ;
    dct:isReferencedBy F2021L00319: ;
    rdfs:comment "Part 2 Variation suspension and revocation of export permit - Abrievated Graph Key: P206"@en-AU ;
    skos:broader F2021L00319:207,
        F2021L00319:208,
        F2021L00319:209,
        F2021L00319:210 ;
    skos:definition "Part 2 Variation suspension and revocation of export permit"@en-AU ;
    skos:narrower F2021L00319:200 ;
    skos:prefLabel "Part P206"@en-AU ;
    dcat:accessURL <https://www.legislation.gov.au/F2021L00319/2024-04-30/2024-04-30/text/original/epub/OEBPS/document_1/document_1.html#_Toc166158039> ;
    dcat:landingPage "https://www.legislation.gov.au/F2021L00319/2024-04-30/2024-04-30/text/original/epub/OEBPS/document_1/document_1.html#_Toc166158039"^^xsd:anyURI ;
    dcat:theme legcons:Part .

F2021L00319:217 a legcons:Division,
        owl:Class,
        dcat:Resource ;
    rdfs:label "Division - D217 Division 1 General"@en-AU ;
    dct:hasPart F2021L00319:218,
        F2021L00319:219,
        F2021L00319:220,
        F2021L00319:221 ;
    dct:isPartOf F2021L00319:216 ;
    dct:isReferencedBy F2021L00319: ;
    rdfs:comment "Division 1 General - Abrievated Graph Key: D217"@en-AU ;
    skos:broader F2021L00319:218,
        F2021L00319:219,
        F2021L00319:220,
        F2021L00319:221 ;
    skos:definition "Division 1 General"@en-AU ;
    skos:narrower F2021L00319:216 ;
    skos:prefLabel "Division D217"@en-AU ;
    dcat:accessURL <https://www.legislation.gov.au/F2021L00319/2024-04-30/2024-04-30/text/original/epub/OEBPS/document_1/document_1.html#_Toc166158050> ;
    dcat:landingPage "https://www.legislation.gov.au/F2021L00319/2024-04-30/2024-04-30/text/original/epub/OEBPS/document_1/document_1.html#_Toc166158050"^^xsd:anyURI ;
    dcat:theme legcons:Division .

F2021L00319:266 a legcons:Division,
        owl:Class,
        dcat:Resource ;
    rdfs:label "Division - D266 Division 2 Conduct of audit"@en-AU ;
    dct:hasPart F2021L00319:267,
        F2021L00319:268,
        F2021L00319:269,
        F2021L00319:270 ;
    dct:isPartOf F2021L00319:263 ;
    dct:isReferencedBy F2021L00319: ;
    rdfs:comment "Division 2 Conduct of audit - Abrievated Graph Key: D266"@en-AU ;
    skos:broader F2021L00319:267,
        F2021L00319:268,
        F2021L00319:269,
        F2021L00319:270 ;
    skos:definition "Division 2 Conduct of audit"@en-AU ;
    skos:narrower F2021L00319:263 ;
    skos:prefLabel "Division D266"@en-AU ;
    dcat:accessURL <https://www.legislation.gov.au/F2021L00319/2024-04-30/2024-04-30/text/original/epub/OEBPS/document_1/document_1.html#_Toc166158099> ;
    dcat:landingPage "https://www.legislation.gov.au/F2021L00319/2024-04-30/2024-04-30/text/original/epub/OEBPS/document_1/document_1.html#_Toc166158099"^^xsd:anyURI ;
    dcat:theme legcons:Division .

F2021L00319:293 a legcons:Division,
        owl:Class,
        dcat:Resource ;
    rdfs:label "Division - D293 Division 5 Suspension of accreditation"@en-AU ;
    dct:hasPart F2021L00319:294,
        F2021L00319:295,
        F2021L00319:296,
        F2021L00319:297 ;
    dct:isPartOf F2021L00319:277 ;
    dct:isReferencedBy F2021L00319: ;
    rdfs:comment "Division 5 Suspension of accreditation - Abrievated Graph Key: D293"@en-AU ;
    skos:broader F2021L00319:294,
        F2021L00319:295,
        F2021L00319:296,
        F2021L00319:297 ;
    skos:definition "Division 5 Suspension of accreditation"@en-AU ;
    skos:narrower F2021L00319:277 ;
    skos:prefLabel "Division D293"@en-AU ;
    dcat:accessURL <https://www.legislation.gov.au/F2021L00319/2024-04-30/2024-04-30/text/original/epub/OEBPS/document_1/document_1.html#_Toc166158126> ;
    dcat:landingPage "https://www.legislation.gov.au/F2021L00319/2024-04-30/2024-04-30/text/original/epub/OEBPS/document_1/document_1.html#_Toc166158126"^^xsd:anyURI ;
    dcat:theme legcons:Division .

F2021L00319:35 a legcons:Division,
        owl:Class,
        dcat:Resource ;
    rdfs:label "Division - D35 Division 2 Prescribed livestock"@en-AU ;
    dct:hasPart F2021L00319:36,
        F2021L00319:37,
        F2021L00319:38,
        F2021L00319:39 ;
    dct:isPartOf F2021L00319:9 ;
    dct:isReferencedBy F2021L00319: ;
    rdfs:comment "Division 2 Prescribed livestock - Abrievated Graph Key: D35"@en-AU ;
    skos:broader F2021L00319:36,
        F2021L00319:37,
        F2021L00319:38,
        F2021L00319:39 ;
    skos:definition "Division 2 Prescribed livestock"@en-AU ;
    skos:narrower F2021L00319:9 ;
    skos:prefLabel "Division D35"@en-AU ;
    dcat:accessURL <https://www.legislation.gov.au/F2021L00319/2024-04-30/2024-04-30/text/original/epub/OEBPS/document_1/document_1.html#_Toc166157868> ;
    dcat:landingPage "https://www.legislation.gov.au/F2021L00319/2024-04-30/2024-04-30/text/original/epub/OEBPS/document_1/document_1.html#_Toc166157868"^^xsd:anyURI ;
    dcat:theme legcons:Division .

F2021L00319:384 a legcons:Division,
        owl:Class,
        dcat:Resource ;
    rdfs:label "Division - D384 Division 1 Notices of intention to export"@en-AU ;
    dct:hasPart F2021L00319:385,
        F2021L00319:386,
        F2021L00319:387,
        F2021L00319:388 ;
    dct:isPartOf F2021L00319:383 ;
    dct:isReferencedBy F2021L00319: ;
    rdfs:comment "Division 1 Notices of intention to export - Abrievated Graph Key: D384"@en-AU ;
    skos:broader F2021L00319:385,
        F2021L00319:386,
        F2021L00319:387,
        F2021L00319:388 ;
    skos:definition "Division 1 Notices of intention to export"@en-AU ;
    skos:narrower F2021L00319:383 ;
    skos:prefLabel "Division D384"@en-AU ;
    dcat:accessURL <https://www.legislation.gov.au/F2021L00319/2024-04-30/2024-04-30/text/original/epub/OEBPS/document_1/document_1.html#_Toc166158217> ;
    dcat:landingPage "https://www.legislation.gov.au/F2021L00319/2024-04-30/2024-04-30/text/original/epub/OEBPS/document_1/document_1.html#_Toc166158217"^^xsd:anyURI ;
    dcat:theme legcons:Division .

F2021L00319:427 a legcons:Endnotes,
        owl:Class,
        dcat:Resource ;
    rdfs:label "Endnotes - E427 Endnotes"@en-AU ;
    dct:hasPart F2021L00319:428,
        F2021L00319:429,
        F2021L00319:430,
        F2021L00319:431 ;
    dct:isPartOf F2021L00319:373 ;
    dct:isReferencedBy F2021L00319: ;
    rdfs:comment "Endnotes - Abrievated Graph Key: E427"@en-AU ;
    skos:broader F2021L00319:428,
        F2021L00319:429,
        F2021L00319:430,
        F2021L00319:431 ;
    skos:definition "Endnotes"@en-AU ;
    skos:narrower F2021L00319:373 ;
    skos:prefLabel "Endnotes E427"@en-AU ;
    dcat:accessURL <https://www.legislation.gov.au/F2021L00319/2024-04-30/2024-04-30/text/original/epub/OEBPS/document_1/document_1.html#_Toc166158260> ;
    dcat:landingPage "https://www.legislation.gov.au/F2021L00319/2024-04-30/2024-04-30/text/original/epub/OEBPS/document_1/document_1.html#_Toc166158260"^^xsd:anyURI ;
    dcat:theme legcons:Endnotes .

F2021L00319:135 a legcons:Division,
        owl:Class,
        dcat:Resource ;
    rdfs:label "Division - D135 Division 2 General conditions"@en-AU ;
    dct:hasPart F2021L00319:136,
        F2021L00319:137,
        F2021L00319:138,
        F2021L00319:139,
        F2021L00319:140 ;
    dct:isPartOf F2021L00319:132 ;
    dct:isReferencedBy F2021L00319: ;
    rdfs:comment "Division 2 General conditions - Abrievated Graph Key: D135"@en-AU ;
    skos:broader F2021L00319:136,
        F2021L00319:137,
        F2021L00319:138,
        F2021L00319:139,
        F2021L00319:140 ;
    skos:definition "Division 2 General conditions"@en-AU ;
    skos:narrower F2021L00319:132 ;
    skos:prefLabel "Division D135"@en-AU ;
    dcat:accessURL <https://www.legislation.gov.au/F2021L00319/2024-04-30/2024-04-30/text/original/epub/OEBPS/document_1/document_1.html#_Toc166157968> ;
    dcat:landingPage "https://www.legislation.gov.au/F2021L00319/2024-04-30/2024-04-30/text/original/epub/OEBPS/document_1/document_1.html#_Toc166157968"^^xsd:anyURI ;
    dcat:theme legcons:Division .

F2021L00319:183 a legcons:Division,
        owl:Class,
        dcat:Resource ;
    rdfs:label "Division - D183 Division 1 Approval of ESCAS"@en-AU ;
    dct:hasPart F2021L00319:184,
        F2021L00319:185,
        F2021L00319:186,
        F2021L00319:187,
        F2021L00319:188 ;
    dct:isPartOf F2021L00319:125 ;
    dct:isReferencedBy F2021L00319: ;
    rdfs:comment "Division 1 Approval of ESCAS - Abrievated Graph Key: D183"@en-AU ;
    skos:broader F2021L00319:184,
        F2021L00319:185,
        F2021L00319:186,
        F2021L00319:187,
        F2021L00319:188 ;
    skos:definition "Division 1 Approval of ESCAS"@en-AU ;
    skos:narrower F2021L00319:125 ;
    skos:prefLabel "Division D183"@en-AU ;
    dcat:accessURL <https://www.legislation.gov.au/F2021L00319/2024-04-30/2024-04-30/text/original/epub/OEBPS/document_1/document_1.html#_Toc166158016> ;
    dcat:landingPage "https://www.legislation.gov.au/F2021L00319/2024-04-30/2024-04-30/text/original/epub/OEBPS/document_1/document_1.html#_Toc166158016"^^xsd:anyURI ;
    dcat:theme legcons:Division .

F2021L00319:223 a legcons:Subdivision,
        owl:Class,
        dcat:Resource ;
    rdfs:label "Subdivision - S223 Subdivision APrescribed livestock"@en-AU ;
    dct:hasPart F2021L00319:224,
        F2021L00319:225,
        F2021L00319:226,
        F2021L00319:227,
        F2021L00319:228 ;
    dct:isPartOf F2021L00319:222 ;
    dct:isReferencedBy F2021L00319: ;
    rdfs:comment "Subdivision APrescribed livestock - Abrievated Graph Key: S223"@en-AU ;
    skos:broader F2021L00319:224,
        F2021L00319:225,
        F2021L00319:226,
        F2021L00319:227,
        F2021L00319:228 ;
    skos:definition "Subdivision APrescribed livestock"@en-AU ;
    skos:narrower F2021L00319:222 ;
    skos:prefLabel "Subdivision S223"@en-AU ;
    dcat:accessURL <https://www.legislation.gov.au/F2021L00319/2024-04-30/2024-04-30/text/original/epub/OEBPS/document_1/document_1.html#_Toc166158056> ;
    dcat:landingPage "https://www.legislation.gov.au/F2021L00319/2024-04-30/2024-04-30/text/original/epub/OEBPS/document_1/document_1.html#_Toc166158056"^^xsd:anyURI ;
    dcat:theme legcons:Subdivision .

F2021L00319:229 a legcons:Subdivision,
        owl:Class,
        dcat:Resource ;
    rdfs:label "Subdivision - S229 Subdivision BPrescribed live animals"@en-AU ;
    dct:hasPart F2021L00319:230,
        F2021L00319:231,
        F2021L00319:232,
        F2021L00319:233,
        F2021L00319:234 ;
    dct:isPartOf F2021L00319:222 ;
    dct:isReferencedBy F2021L00319: ;
    rdfs:comment "Subdivision BPrescribed live animals - Abrievated Graph Key: S229"@en-AU ;
    skos:broader F2021L00319:230,
        F2021L00319:231,
        F2021L00319:232,
        F2021L00319:233,
        F2021L00319:234 ;
    skos:definition "Subdivision BPrescribed live animals"@en-AU ;
    skos:narrower F2021L00319:222 ;
    skos:prefLabel "Subdivision S229"@en-AU ;
    dcat:accessURL <https://www.legislation.gov.au/F2021L00319/2024-04-30/2024-04-30/text/original/epub/OEBPS/document_1/document_1.html#_Toc166158062> ;
    dcat:landingPage "https://www.legislation.gov.au/F2021L00319/2024-04-30/2024-04-30/text/original/epub/OEBPS/document_1/document_1.html#_Toc166158062"^^xsd:anyURI ;
    dcat:theme legcons:Subdivision .

F2021L00319:262 a legcons:Chapter,
        owl:Class,
        dcat:Resource ;
    rdfs:label "Chapter - C262 Chapter 9 Powers and officials"@en-AU ;
    dct:hasPart F2021L00319:263,
        F2021L00319:271,
        F2021L00319:277,
        F2021L00319:310,
        F2021L00319:341,
        F2021L00319:344 ;
    dct:isReferencedBy F2021L00319: ;
    rdfs:comment "Chapter 9 Powers and officials - Abrievated Graph Key: C262"@en-AU ;
    skos:broader F2021L00319:263,
        F2021L00319:271,
        F2021L00319:277,
        F2021L00319:310,
        F2021L00319:341,
        F2021L00319:344 ;
    skos:definition "Chapter 9 Powers and officials"@en-AU ;
    skos:prefLabel "Chapter C262"@en-AU ;
    dcat:accessURL <https://www.legislation.gov.au/F2021L00319/2024-04-30/2024-04-30/text/original/epub/OEBPS/document_1/document_1.html#_Toc166158095> ;
    dcat:landingPage "https://www.legislation.gov.au/F2021L00319/2024-04-30/2024-04-30/text/original/epub/OEBPS/document_1/document_1.html#_Toc166158095"^^xsd:anyURI ;
    dcat:theme legcons:Chapter .

F2021L00319:310 a legcons:Part,
        owl:Class,
        dcat:Resource ;
    rdfs:label "Part - P310 Part 4 Approved export programs"@en-AU ;
    dct:hasPart F2021L00319:311,
        F2021L00319:313,
        F2021L00319:331,
        F2021L00319:335,
        F2021L00319:338 ;
    dct:isPartOf F2021L00319:262 ;
    dct:isReferencedBy F2021L00319: ;
    rdfs:comment "Part 4 Approved export programs - Abrievated Graph Key: P310"@en-AU ;
    skos:broader F2021L00319:311,
        F2021L00319:313,
        F2021L00319:331,
        F2021L00319:335,
        F2021L00319:338 ;
    skos:definition "Part 4 Approved export programs"@en-AU ;
    skos:narrower F2021L00319:262 ;
    skos:prefLabel "Part P310"@en-AU ;
    dcat:accessURL <https://www.legislation.gov.au/F2021L00319/2024-04-30/2024-04-30/text/original/epub/OEBPS/document_1/document_1.html#_Toc166158143> ;
    dcat:landingPage "https://www.legislation.gov.au/F2021L00319/2024-04-30/2024-04-30/text/original/epub/OEBPS/document_1/document_1.html#_Toc166158143"^^xsd:anyURI ;
    dcat:theme legcons:Part .

F2021L00319:313 a legcons:Division,
        owl:Class,
        dcat:Resource ;
    rdfs:label "Division - D313 Division 2 Exporters approved export programs"@en-AU ;
    dct:hasPart F2021L00319:314,
        F2021L00319:318,
        F2021L00319:322,
        F2021L00319:326,
        F2021L00319:329 ;
    dct:isPartOf F2021L00319:310 ;
    dct:isReferencedBy F2021L00319: ;
    rdfs:comment "Division 2 Exporters approved export programs - Abrievated Graph Key: D313"@en-AU ;
    skos:broader F2021L00319:314,
        F2021L00319:318,
        F2021L00319:322,
        F2021L00319:326,
        F2021L00319:329 ;
    skos:definition "Division 2 Exporters approved export programs"@en-AU ;
    skos:narrower F2021L00319:310 ;
    skos:prefLabel "Division D313"@en-AU ;
    dcat:accessURL <https://www.legislation.gov.au/F2021L00319/2024-04-30/2024-04-30/text/original/epub/OEBPS/document_1/document_1.html#_Toc166158146> ;
    dcat:landingPage "https://www.legislation.gov.au/F2021L00319/2024-04-30/2024-04-30/text/original/epub/OEBPS/document_1/document_1.html#_Toc166158146"^^xsd:anyURI ;
    dcat:theme legcons:Division .

F2021L00319:350 a legcons:Chapter,
        owl:Class,
        dcat:Resource ;
    rdfs:label "Chapter - C350 Chapter 11 Miscellaneous"@en-AU ;
    dct:hasPart F2021L00319:351,
        F2021L00319:353,
        F2021L00319:364,
        F2021L00319:366,
        F2021L00319:369,
        F2021L00319:371 ;
    dct:isReferencedBy F2021L00319: ;
    rdfs:comment "Chapter 11 Miscellaneous - Abrievated Graph Key: C350"@en-AU ;
    skos:broader F2021L00319:351,
        F2021L00319:353,
        F2021L00319:364,
        F2021L00319:366,
        F2021L00319:369,
        F2021L00319:371 ;
    skos:definition "Chapter 11 Miscellaneous"@en-AU ;
    skos:prefLabel "Chapter C350"@en-AU ;
    dcat:accessURL <https://www.legislation.gov.au/F2021L00319/2024-04-30/2024-04-30/text/original/epub/OEBPS/document_1/document_1.html#_Toc166158183> ;
    dcat:landingPage "https://www.legislation.gov.au/F2021L00319/2024-04-30/2024-04-30/text/original/epub/OEBPS/document_1/document_1.html#_Toc166158183"^^xsd:anyURI ;
    dcat:theme legcons:Chapter .

F2021L00319:421 a legcons:Part,
        owl:Class,
        dcat:Resource ;
    rdfs:label "Part - P421 Part 8 Amendments made by the Export Control Animals Amendment Improving Regulatory Outcomes Rules 2023"@en-AU ;
    dct:hasPart F2021L00319:422,
        F2021L00319:423,
        F2021L00319:424,
        F2021L00319:425,
        F2021L00319:426 ;
    dct:isPartOf F2021L00319:373 ;
    dct:isReferencedBy F2021L00319: ;
    rdfs:comment "Part 8 Amendments made by the Export Control Animals Amendment Improving Regulatory Outcomes Rules 2023 - Abrievated Graph Key: P421"@en-AU ;
    skos:broader F2021L00319:422,
        F2021L00319:423,
        F2021L00319:424,
        F2021L00319:425,
        F2021L00319:426 ;
    skos:definition "Part 8 Amendments made by the Export Control Animals Amendment Improving Regulatory Outcomes Rules 2023"@en-AU ;
    skos:narrower F2021L00319:373 ;
    skos:prefLabel "Part P421"@en-AU ;
    dcat:accessURL <https://www.legislation.gov.au/F2021L00319/2024-04-30/2024-04-30/text/original/epub/OEBPS/document_1/document_1.html#_Toc166158254> ;
    dcat:landingPage "https://www.legislation.gov.au/F2021L00319/2024-04-30/2024-04-30/text/original/epub/OEBPS/document_1/document_1.html#_Toc166158254"^^xsd:anyURI ;
    dcat:theme legcons:Part .

F2021L00319:78 a legcons:Division,
        owl:Class,
        dcat:Resource ;
    rdfs:label "Division - D78 Division 2 Conditions of approved arrangement"@en-AU ;
    dct:hasPart F2021L00319:79,
        F2021L00319:80,
        F2021L00319:81,
        F2021L00319:82,
        F2021L00319:83 ;
    dct:isPartOf F2021L00319:75 ;
    dct:isReferencedBy F2021L00319: ;
    rdfs:comment "Division 2 Conditions of approved arrangement - Abrievated Graph Key: D78"@en-AU ;
    skos:broader F2021L00319:79,
        F2021L00319:80,
        F2021L00319:81,
        F2021L00319:82,
        F2021L00319:83 ;
    skos:definition "Division 2 Conditions of approved arrangement"@en-AU ;
    skos:narrower F2021L00319:75 ;
    skos:prefLabel "Division D78"@en-AU ;
    dcat:accessURL <https://www.legislation.gov.au/F2021L00319/2024-04-30/2024-04-30/text/original/epub/OEBPS/document_1/document_1.html#_Toc166157911> ;
    dcat:landingPage "https://www.legislation.gov.au/F2021L00319/2024-04-30/2024-04-30/text/original/epub/OEBPS/document_1/document_1.html#_Toc166157911"^^xsd:anyURI ;
    dcat:theme legcons:Division .

F2021L00319:93 a legcons:Division,
        owl:Class,
        dcat:Resource ;
    rdfs:label "Division - D93 Division 1 Requirements for approval"@en-AU ;
    dct:hasPart F2021L00319:94,
        F2021L00319:95,
        F2021L00319:96,
        F2021L00319:97,
        F2021L00319:98 ;
    dct:isPartOf F2021L00319:92 ;
    dct:isReferencedBy F2021L00319: ;
    rdfs:comment "Division 1 Requirements for approval - Abrievated Graph Key: D93"@en-AU ;
    skos:broader F2021L00319:94,
        F2021L00319:95,
        F2021L00319:96,
        F2021L00319:97,
        F2021L00319:98 ;
    skos:definition "Division 1 Requirements for approval"@en-AU ;
    skos:narrower F2021L00319:92 ;
    skos:prefLabel "Division D93"@en-AU ;
    dcat:accessURL <https://www.legislation.gov.au/F2021L00319/2024-04-30/2024-04-30/text/original/epub/OEBPS/document_1/document_1.html#_Toc166157926> ;
    dcat:landingPage "https://www.legislation.gov.au/F2021L00319/2024-04-30/2024-04-30/text/original/epub/OEBPS/document_1/document_1.html#_Toc166157926"^^xsd:anyURI ;
    dcat:theme legcons:Division .

F2021L00319:99 a legcons:Division,
        owl:Class,
        dcat:Resource ;
    rdfs:label "Division - D99 Division 2 Conditions of approved arrangement"@en-AU ;
    dct:hasPart F2021L00319:100,
        F2021L00319:101,
        F2021L00319:102,
        F2021L00319:103,
        F2021L00319:104 ;
    dct:isPartOf F2021L00319:92 ;
    dct:isReferencedBy F2021L00319: ;
    rdfs:comment "Division 2 Conditions of approved arrangement - Abrievated Graph Key: D99"@en-AU ;
    skos:broader F2021L00319:100,
        F2021L00319:101,
        F2021L00319:102,
        F2021L00319:103,
        F2021L00319:104 ;
    skos:definition "Division 2 Conditions of approved arrangement"@en-AU ;
    skos:narrower F2021L00319:92 ;
    skos:prefLabel "Division D99"@en-AU ;
    dcat:accessURL <https://www.legislation.gov.au/F2021L00319/2024-04-30/2024-04-30/text/original/epub/OEBPS/document_1/document_1.html#_Toc166157932> ;
    dcat:landingPage "https://www.legislation.gov.au/F2021L00319/2024-04-30/2024-04-30/text/original/epub/OEBPS/document_1/document_1.html#_Toc166157932"^^xsd:anyURI ;
    dcat:theme legcons:Division .

F2021L00319:1 a legcons:Chapter,
        owl:Class,
        dcat:Resource ;
    rdfs:label "Chapter - C1 Chapter 1 Preliminary"@en-AU ;
    dct:hasPart F2021L00319:2,
        F2021L00319:3,
        F2021L00319:4,
        F2021L00319:5,
        F2021L00319:6,
        F2021L00319:7,
        F2021L00319:8 ;
    dct:isReferencedBy F2021L00319: ;
    rdfs:comment "Chapter 1 Preliminary - Abrievated Graph Key: C1"@en-AU ;
    skos:broader F2021L00319:2,
        F2021L00319:3,
        F2021L00319:4,
        F2021L00319:5,
        F2021L00319:6,
        F2021L00319:7,
        F2021L00319:8 ;
    skos:definition "Chapter 1 Preliminary"@en-AU ;
    skos:prefLabel "Chapter C1"@en-AU ;
    dcat:accessURL <https://www.legislation.gov.au/F2021L00319/2024-04-30/2024-04-30/text/original/epub/OEBPS/document_1/document_1.html#_Toc166157834> ;
    dcat:landingPage "https://www.legislation.gov.au/F2021L00319/2024-04-30/2024-04-30/text/original/epub/OEBPS/document_1/document_1.html#_Toc166157834"^^xsd:anyURI ;
    dcat:theme legcons:Chapter .

F2021L00319:10 a legcons:Part,
        owl:Class,
        dcat:Resource ;
    rdfs:label "Part - P10 Part 1 Goods"@en-AU ;
    dct:hasPart F2021L00319:11,
        F2021L00319:13,
        F2021L00319:14,
        F2021L00319:15,
        F2021L00319:16,
        F2021L00319:17 ;
    dct:isPartOf F2021L00319:9 ;
    dct:isReferencedBy F2021L00319: ;
    rdfs:comment "Part 1 Goods - Abrievated Graph Key: P10"@en-AU ;
    skos:broader F2021L00319:11,
        F2021L00319:13,
        F2021L00319:14,
        F2021L00319:15,
        F2021L00319:16,
        F2021L00319:17 ;
    skos:definition "Part 1 Goods"@en-AU ;
    skos:narrower F2021L00319:9 ;
    skos:prefLabel "Part P10"@en-AU ;
    dcat:accessURL <https://www.legislation.gov.au/F2021L00319/2024-04-30/2024-04-30/text/original/epub/OEBPS/document_1/document_1.html#_Toc166157843> ;
    dcat:landingPage "https://www.legislation.gov.au/F2021L00319/2024-04-30/2024-04-30/text/original/epub/OEBPS/document_1/document_1.html#_Toc166157843"^^xsd:anyURI ;
    dcat:theme legcons:Part .

F2021L00319:236 a legcons:Division,
        owl:Class,
        dcat:Resource ;
    rdfs:label "Division - D236 Division 1 Marks that are official marks"@en-AU ;
    dct:hasPart F2021L00319:237,
        F2021L00319:238,
        F2021L00319:239,
        F2021L00319:240,
        F2021L00319:241,
        F2021L00319:242 ;
    dct:isPartOf F2021L00319:235 ;
    dct:isReferencedBy F2021L00319: ;
    rdfs:comment "Division 1 Marks that are official marks - Abrievated Graph Key: D236"@en-AU ;
    skos:broader F2021L00319:237,
        F2021L00319:238,
        F2021L00319:239,
        F2021L00319:240,
        F2021L00319:241,
        F2021L00319:242 ;
    skos:definition "Division 1 Marks that are official marks"@en-AU ;
    skos:narrower F2021L00319:235 ;
    skos:prefLabel "Division D236"@en-AU ;
    dcat:accessURL <https://www.legislation.gov.au/F2021L00319/2024-04-30/2024-04-30/text/original/epub/OEBPS/document_1/document_1.html#_Toc166158069> ;
    dcat:landingPage "https://www.legislation.gov.au/F2021L00319/2024-04-30/2024-04-30/text/original/epub/OEBPS/document_1/document_1.html#_Toc166158069"^^xsd:anyURI ;
    dcat:theme legcons:Division .

F2021L00319:255 a legcons:Division,
        owl:Class,
        dcat:Resource ;
    rdfs:label "Division - D255 Division 3 Official marking devices"@en-AU ;
    dct:hasPart F2021L00319:256,
        F2021L00319:257,
        F2021L00319:258,
        F2021L00319:259,
        F2021L00319:260,
        F2021L00319:261 ;
    dct:isPartOf F2021L00319:235 ;
    dct:isReferencedBy F2021L00319: ;
    rdfs:comment "Division 3 Official marking devices - Abrievated Graph Key: D255"@en-AU ;
    skos:broader F2021L00319:256,
        F2021L00319:257,
        F2021L00319:258,
        F2021L00319:259,
        F2021L00319:260,
        F2021L00319:261 ;
    skos:definition "Division 3 Official marking devices"@en-AU ;
    skos:narrower F2021L00319:235 ;
    skos:prefLabel "Division D255"@en-AU ;
    dcat:accessURL <https://www.legislation.gov.au/F2021L00319/2024-04-30/2024-04-30/text/original/epub/OEBPS/document_1/document_1.html#_Toc166158088> ;
    dcat:landingPage "https://www.legislation.gov.au/F2021L00319/2024-04-30/2024-04-30/text/original/epub/OEBPS/document_1/document_1.html#_Toc166158088"^^xsd:anyURI ;
    dcat:theme legcons:Division .

F2021L00319:280 a legcons:Division,
        owl:Class,
        dcat:Resource ;
    rdfs:label "Division - D280 Division 2 Application for accreditation"@en-AU ;
    dct:hasPart F2021L00319:281,
        F2021L00319:282,
        F2021L00319:283,
        F2021L00319:284,
        F2021L00319:285,
        F2021L00319:286 ;
    dct:isPartOf F2021L00319:277 ;
    dct:isReferencedBy F2021L00319: ;
    rdfs:comment "Division 2 Application for accreditation - Abrievated Graph Key: D280"@en-AU ;
    skos:broader F2021L00319:281,
        F2021L00319:282,
        F2021L00319:283,
        F2021L00319:284,
        F2021L00319:285,
        F2021L00319:286 ;
    skos:definition "Division 2 Application for accreditation"@en-AU ;
    skos:narrower F2021L00319:277 ;
    skos:prefLabel "Division D280"@en-AU ;
    dcat:accessURL <https://www.legislation.gov.au/F2021L00319/2024-04-30/2024-04-30/text/original/epub/OEBPS/document_1/document_1.html#_Toc166158113> ;
    dcat:landingPage "https://www.legislation.gov.au/F2021L00319/2024-04-30/2024-04-30/text/original/epub/OEBPS/document_1/document_1.html#_Toc166158113"^^xsd:anyURI ;
    dcat:theme legcons:Division .

F2021L00319:52 a legcons:Part,
        owl:Class,
        dcat:Resource ;
    rdfs:label "Part - P52 Part 3 Conditions of registration"@en-AU ;
    dct:hasPart F2021L00319:53,
        F2021L00319:54,
        F2021L00319:55,
        F2021L00319:56,
        F2021L00319:57,
        F2021L00319:58 ;
    dct:isPartOf F2021L00319:43 ;
    dct:isReferencedBy F2021L00319: ;
    rdfs:comment "Part 3 Conditions of registration - Abrievated Graph Key: P52"@en-AU ;
    skos:broader F2021L00319:53,
        F2021L00319:54,
        F2021L00319:55,
        F2021L00319:56,
        F2021L00319:57,
        F2021L00319:58 ;
    skos:definition "Part 3 Conditions of registration"@en-AU ;
    skos:narrower F2021L00319:43 ;
    skos:prefLabel "Part P52"@en-AU ;
    dcat:accessURL <https://www.legislation.gov.au/F2021L00319/2024-04-30/2024-04-30/text/original/epub/OEBPS/document_1/document_1.html#_Toc166157885> ;
    dcat:landingPage "https://www.legislation.gov.au/F2021L00319/2024-04-30/2024-04-30/text/original/epub/OEBPS/document_1/document_1.html#_Toc166157885"^^xsd:anyURI ;
    dcat:theme legcons:Part .

F2021L00319:75 a legcons:Part,
        owl:Class,
        dcat:Resource ;
    rdfs:label "Part - P75 Part 1 Approved arrangements other than for exporter supply chain assurance operations"@en-AU ;
    dct:hasPart F2021L00319:76,
        F2021L00319:78,
        F2021L00319:84,
        F2021L00319:86,
        F2021L00319:88,
        F2021L00319:90 ;
    dct:isPartOf F2021L00319:74 ;
    dct:isReferencedBy F2021L00319: ;
    rdfs:comment "Part 1 Approved arrangements other than for exporter supply chain assurance operations - Abrievated Graph Key: P75"@en-AU ;
    skos:broader F2021L00319:76,
        F2021L00319:78,
        F2021L00319:84,
        F2021L00319:86,
        F2021L00319:88,
        F2021L00319:90 ;
    skos:definition "Part 1 Approved arrangements other than for exporter supply chain assurance operations"@en-AU ;
    skos:narrower F2021L00319:74 ;
    skos:prefLabel "Part P75"@en-AU ;
    dcat:accessURL <https://www.legislation.gov.au/F2021L00319/2024-04-30/2024-04-30/text/original/epub/OEBPS/document_1/document_1.html#_Toc166157908> ;
    dcat:landingPage "https://www.legislation.gov.au/F2021L00319/2024-04-30/2024-04-30/text/original/epub/OEBPS/document_1/document_1.html#_Toc166157908"^^xsd:anyURI ;
    dcat:theme legcons:Part .

F2021L00319:132 a legcons:Part,
        owl:Class,
        dcat:Resource ;
    rdfs:label "Part - P132 Part 2 Conditions of livestock export licence"@en-AU ;
    dct:hasPart F2021L00319:133,
        F2021L00319:135,
        F2021L00319:141,
        F2021L00319:144,
        F2021L00319:165,
        F2021L00319:166,
        F2021L00319:167 ;
    dct:isPartOf F2021L00319:125 ;
    dct:isReferencedBy F2021L00319: ;
    rdfs:comment "Part 2 Conditions of livestock export licence - Abrievated Graph Key: P132"@en-AU ;
    skos:broader F2021L00319:133,
        F2021L00319:135,
        F2021L00319:141,
        F2021L00319:144,
        F2021L00319:165,
        F2021L00319:166,
        F2021L00319:167 ;
    skos:definition "Part 2 Conditions of livestock export licence"@en-AU ;
    skos:narrower F2021L00319:125 ;
    skos:prefLabel "Part P132"@en-AU ;
    dcat:accessURL <https://www.legislation.gov.au/F2021L00319/2024-04-30/2024-04-30/text/original/epub/OEBPS/document_1/document_1.html#_Toc166157965> ;
    dcat:landingPage "https://www.legislation.gov.au/F2021L00319/2024-04-30/2024-04-30/text/original/epub/OEBPS/document_1/document_1.html#_Toc166157965"^^xsd:anyURI ;
    dcat:theme legcons:Part .

F2021L00319:27 a legcons:Division,
        owl:Class,
        dcat:Resource ;
    rdfs:label "Division - D27 Division 1 General"@en-AU ;
    dct:hasPart F2021L00319:28,
        F2021L00319:29,
        F2021L00319:30,
        F2021L00319:31,
        F2021L00319:32,
        F2021L00319:33,
        F2021L00319:34 ;
    dct:isPartOf F2021L00319:9 ;
    dct:isReferencedBy F2021L00319: ;
    rdfs:comment "Division 1 General - Abrievated Graph Key: D27"@en-AU ;
    skos:broader F2021L00319:28,
        F2021L00319:29,
        F2021L00319:30,
        F2021L00319:31,
        F2021L00319:32,
        F2021L00319:33,
        F2021L00319:34 ;
    skos:definition "Division 1 General"@en-AU ;
    skos:narrower F2021L00319:9 ;
    skos:prefLabel "Division D27"@en-AU ;
    dcat:accessURL <https://www.legislation.gov.au/F2021L00319/2024-04-30/2024-04-30/text/original/epub/OEBPS/document_1/document_1.html#_Toc166157860> ;
    dcat:landingPage "https://www.legislation.gov.au/F2021L00319/2024-04-30/2024-04-30/text/original/epub/OEBPS/document_1/document_1.html#_Toc166157860"^^xsd:anyURI ;
    dcat:theme legcons:Division .

F2021L00319:397 a legcons:Division,
        owl:Class,
        dcat:Resource ;
    rdfs:label "Division - D397 Division 1 Accredited veterinarians"@en-AU ;
    dct:hasPart F2021L00319:398,
        F2021L00319:399,
        F2021L00319:400,
        F2021L00319:401,
        F2021L00319:402,
        F2021L00319:403,
        F2021L00319:404 ;
    dct:isPartOf F2021L00319:396 ;
    dct:isReferencedBy F2021L00319: ;
    rdfs:comment "Division 1 Accredited veterinarians - Abrievated Graph Key: D397"@en-AU ;
    skos:broader F2021L00319:398,
        F2021L00319:399,
        F2021L00319:400,
        F2021L00319:401,
        F2021L00319:402,
        F2021L00319:403,
        F2021L00319:404 ;
    skos:definition "Division 1 Accredited veterinarians"@en-AU ;
    skos:narrower F2021L00319:396 ;
    skos:prefLabel "Division D397"@en-AU ;
    dcat:accessURL <https://www.legislation.gov.au/F2021L00319/2024-04-30/2024-04-30/text/original/epub/OEBPS/document_1/document_1.html#_Toc166158230> ;
    dcat:landingPage "https://www.legislation.gov.au/F2021L00319/2024-04-30/2024-04-30/text/original/epub/OEBPS/document_1/document_1.html#_Toc166158230"^^xsd:anyURI ;
    dcat:theme legcons:Division .

F2021L00319:406 a legcons:Subdivision,
        owl:Class,
        dcat:Resource ;
    rdfs:label "Subdivision - S406 Subdivision AExporters approved export programs"@en-AU ;
    dct:hasPart F2021L00319:407,
        F2021L00319:408,
        F2021L00319:409,
        F2021L00319:410,
        F2021L00319:411,
        F2021L00319:412,
        F2021L00319:413 ;
    dct:isPartOf F2021L00319:405 ;
    dct:isReferencedBy F2021L00319: ;
    rdfs:comment "Subdivision AExporters approved export programs - Abrievated Graph Key: S406"@en-AU ;
    skos:broader F2021L00319:407,
        F2021L00319:408,
        F2021L00319:409,
        F2021L00319:410,
        F2021L00319:411,
        F2021L00319:412,
        F2021L00319:413 ;
    skos:definition "Subdivision AExporters approved export programs"@en-AU ;
    skos:narrower F2021L00319:405 ;
    skos:prefLabel "Subdivision S406"@en-AU ;
    dcat:accessURL <https://www.legislation.gov.au/F2021L00319/2024-04-30/2024-04-30/text/original/epub/OEBPS/document_1/document_1.html#_Toc166158239> ;
    dcat:landingPage "https://www.legislation.gov.au/F2021L00319/2024-04-30/2024-04-30/text/original/epub/OEBPS/document_1/document_1.html#_Toc166158239"^^xsd:anyURI ;
    dcat:theme legcons:Subdivision .

F2021L00319:373 a legcons:Chapter,
        owl:Class,
        dcat:Resource ;
    rdfs:label "Chapter - C373 Chapter 12 Application saving and transitional provisions"@en-AU ;
    dct:hasPart F2021L00319:374,
        F2021L00319:376,
        F2021L00319:379,
        F2021L00319:383,
        F2021L00319:396,
        F2021L00319:417,
        F2021L00319:419,
        F2021L00319:421,
        F2021L00319:427 ;
    dct:isReferencedBy F2021L00319: ;
    rdfs:comment "Chapter 12 Application saving and transitional provisions - Abrievated Graph Key: C373"@en-AU ;
    skos:broader F2021L00319:374,
        F2021L00319:376,
        F2021L00319:379,
        F2021L00319:383,
        F2021L00319:396,
        F2021L00319:417,
        F2021L00319:419,
        F2021L00319:421,
        F2021L00319:427 ;
    skos:definition "Chapter 12 Application saving and transitional provisions"@en-AU ;
    skos:prefLabel "Chapter C373"@en-AU ;
    dcat:accessURL <https://www.legislation.gov.au/F2021L00319/2024-04-30/2024-04-30/text/original/epub/OEBPS/document_1/document_1.html#_Toc166158206> ;
    dcat:landingPage "https://www.legislation.gov.au/F2021L00319/2024-04-30/2024-04-30/text/original/epub/OEBPS/document_1/document_1.html#_Toc166158206"^^xsd:anyURI ;
    dcat:theme legcons:Chapter .

F2021L00319:43 a legcons:Chapter,
        owl:Class,
        dcat:Resource ;
    rdfs:label "Chapter - C43 Chapter 4 Registered establishments"@en-AU ;
    dct:hasPart F2021L00319:44,
        F2021L00319:46,
        F2021L00319:52,
        F2021L00319:59,
        F2021L00319:62,
        F2021L00319:64,
        F2021L00319:66,
        F2021L00319:68,
        F2021L00319:72 ;
    dct:isReferencedBy F2021L00319: ;
    rdfs:comment "Chapter 4 Registered establishments - Abrievated Graph Key: C43"@en-AU ;
    skos:broader F2021L00319:44,
        F2021L00319:46,
        F2021L00319:52,
        F2021L00319:59,
        F2021L00319:62,
        F2021L00319:64,
        F2021L00319:66,
        F2021L00319:68,
        F2021L00319:72 ;
    skos:definition "Chapter 4 Registered establishments"@en-AU ;
    skos:prefLabel "Chapter C43"@en-AU ;
    dcat:accessURL <https://www.legislation.gov.au/F2021L00319/2024-04-30/2024-04-30/text/original/epub/OEBPS/document_1/document_1.html#_Toc166157876> ;
    dcat:landingPage "https://www.legislation.gov.au/F2021L00319/2024-04-30/2024-04-30/text/original/epub/OEBPS/document_1/document_1.html#_Toc166157876"^^xsd:anyURI ;
    dcat:theme legcons:Chapter .

F2021L00319:92 a legcons:Part,
        owl:Class,
        dcat:Resource ;
    rdfs:label "Part - P92 Part 2 Approved arrangements for exporter supply chain assurance operations"@en-AU ;
    dct:hasPart F2021L00319:105,
        F2021L00319:107,
        F2021L00319:110,
        F2021L00319:114,
        F2021L00319:116,
        F2021L00319:118,
        F2021L00319:93,
        F2021L00319:99 ;
    dct:isPartOf F2021L00319:74 ;
    dct:isReferencedBy F2021L00319: ;
    rdfs:comment "Part 2 Approved arrangements for exporter supply chain assurance operations - Abrievated Graph Key: P92"@en-AU ;
    skos:broader F2021L00319:105,
        F2021L00319:107,
        F2021L00319:110,
        F2021L00319:114,
        F2021L00319:116,
        F2021L00319:118,
        F2021L00319:93,
        F2021L00319:99 ;
    skos:definition "Part 2 Approved arrangements for exporter supply chain assurance operations"@en-AU ;
    skos:narrower F2021L00319:74 ;
    skos:prefLabel "Part P92"@en-AU ;
    dcat:accessURL <https://www.legislation.gov.au/F2021L00319/2024-04-30/2024-04-30/text/original/epub/OEBPS/document_1/document_1.html#_Toc166157925> ;
    dcat:landingPage "https://www.legislation.gov.au/F2021L00319/2024-04-30/2024-04-30/text/original/epub/OEBPS/document_1/document_1.html#_Toc166157925"^^xsd:anyURI ;
    dcat:theme legcons:Part .

F2021L00319:277 a legcons:Part,
        owl:Class,
        dcat:Resource ;
    rdfs:label "Part - P277 Part 3 Accredited veterinarians"@en-AU ;
    dct:hasPart F2021L00319:278,
        F2021L00319:280,
        F2021L00319:287,
        F2021L00319:290,
        F2021L00319:293,
        F2021L00319:298,
        F2021L00319:301,
        F2021L00319:304,
        F2021L00319:306 ;
    dct:isPartOf F2021L00319:262 ;
    dct:isReferencedBy F2021L00319: ;
    rdfs:comment "Part 3 Accredited veterinarians - Abrievated Graph Key: P277"@en-AU ;
    skos:broader F2021L00319:278,
        F2021L00319:280,
        F2021L00319:287,
        F2021L00319:290,
        F2021L00319:293,
        F2021L00319:298,
        F2021L00319:301,
        F2021L00319:304,
        F2021L00319:306 ;
    skos:definition "Part 3 Accredited veterinarians"@en-AU ;
    skos:narrower F2021L00319:262 ;
    skos:prefLabel "Part P277"@en-AU ;
    dcat:accessURL <https://www.legislation.gov.au/F2021L00319/2024-04-30/2024-04-30/text/original/epub/OEBPS/document_1/document_1.html#_Toc166158110> ;
    dcat:landingPage "https://www.legislation.gov.au/F2021L00319/2024-04-30/2024-04-30/text/original/epub/OEBPS/document_1/document_1.html#_Toc166158110"^^xsd:anyURI ;
    dcat:theme legcons:Part .

F2021L00319:353 a legcons:Part,
        owl:Class,
        dcat:Resource ;
    rdfs:label "Part - P353 Part 2 Records"@en-AU ;
    dct:hasPart F2021L00319:354,
        F2021L00319:355,
        F2021L00319:356,
        F2021L00319:357,
        F2021L00319:358,
        F2021L00319:359,
        F2021L00319:360,
        F2021L00319:361,
        F2021L00319:362,
        F2021L00319:363 ;
    dct:isPartOf F2021L00319:350 ;
    dct:isReferencedBy F2021L00319: ;
    rdfs:comment "Part 2 Records - Abrievated Graph Key: P353"@en-AU ;
    skos:broader F2021L00319:354,
        F2021L00319:355,
        F2021L00319:356,
        F2021L00319:357,
        F2021L00319:358,
        F2021L00319:359,
        F2021L00319:360,
        F2021L00319:361,
        F2021L00319:362,
        F2021L00319:363 ;
    skos:definition "Part 2 Records"@en-AU ;
    skos:narrower F2021L00319:350 ;
    skos:prefLabel "Part P353"@en-AU ;
    dcat:accessURL <https://www.legislation.gov.au/F2021L00319/2024-04-30/2024-04-30/text/original/epub/OEBPS/document_1/document_1.html#_Toc166158186> ;
    dcat:landingPage "https://www.legislation.gov.au/F2021L00319/2024-04-30/2024-04-30/text/original/epub/OEBPS/document_1/document_1.html#_Toc166158186"^^xsd:anyURI ;
    dcat:theme legcons:Part .

F2021L00319:243 a legcons:Division,
        owl:Class,
        dcat:Resource ;
    rdfs:label "Division - D243 Division 2 General rules relating to official marks"@en-AU ;
    dct:hasPart F2021L00319:244,
        F2021L00319:245,
        F2021L00319:246,
        F2021L00319:247,
        F2021L00319:248,
        F2021L00319:249,
        F2021L00319:250,
        F2021L00319:251,
        F2021L00319:252,
        F2021L00319:253,
        F2021L00319:254 ;
    dct:isPartOf F2021L00319:235 ;
    dct:isReferencedBy F2021L00319: ;
    rdfs:comment "Division 2 General rules relating to official marks - Abrievated Graph Key: D243"@en-AU ;
    skos:broader F2021L00319:244,
        F2021L00319:245,
        F2021L00319:246,
        F2021L00319:247,
        F2021L00319:248,
        F2021L00319:249,
        F2021L00319:250,
        F2021L00319:251,
        F2021L00319:252,
        F2021L00319:253,
        F2021L00319:254 ;
    skos:definition "Division 2 General rules relating to official marks"@en-AU ;
    skos:narrower F2021L00319:235 ;
    skos:prefLabel "Division D243"@en-AU ;
    dcat:accessURL <https://www.legislation.gov.au/F2021L00319/2024-04-30/2024-04-30/text/original/epub/OEBPS/document_1/document_1.html#_Toc166158076> ;
    dcat:landingPage "https://www.legislation.gov.au/F2021L00319/2024-04-30/2024-04-30/text/original/epub/OEBPS/document_1/document_1.html#_Toc166158076"^^xsd:anyURI ;
    dcat:theme legcons:Division .

F2021L00319:9 a legcons:Chapter,
        owl:Class,
        dcat:Resource ;
    rdfs:label "Chapter - C9 Chapter 2 Exporting goods"@en-AU ;
    dct:hasPart F2021L00319:10,
        F2021L00319:18,
        F2021L00319:19,
        F2021L00319:20,
        F2021L00319:21,
        F2021L00319:22,
        F2021L00319:23,
        F2021L00319:24,
        F2021L00319:25,
        F2021L00319:26,
        F2021L00319:27,
        F2021L00319:35,
        F2021L00319:40 ;
    dct:isReferencedBy F2021L00319: ;
    rdfs:comment "Chapter 2 Exporting goods - Abrievated Graph Key: C9"@en-AU ;
    skos:broader F2021L00319:10,
        F2021L00319:18,
        F2021L00319:19,
        F2021L00319:20,
        F2021L00319:21,
        F2021L00319:22,
        F2021L00319:23,
        F2021L00319:24,
        F2021L00319:25,
        F2021L00319:26,
        F2021L00319:27,
        F2021L00319:35,
        F2021L00319:40 ;
    skos:definition "Chapter 2 Exporting goods"@en-AU ;
    skos:prefLabel "Chapter C9"@en-AU ;
    dcat:accessURL <https://www.legislation.gov.au/F2021L00319/2024-04-30/2024-04-30/text/original/epub/OEBPS/document_1/document_1.html#_Toc166157842> ;
    dcat:landingPage "https://www.legislation.gov.au/F2021L00319/2024-04-30/2024-04-30/text/original/epub/OEBPS/document_1/document_1.html#_Toc166157842"^^xsd:anyURI ;
    dcat:theme legcons:Chapter .

F2021L00319:144 a legcons:Division,
        owl:Class,
        dcat:Resource ;
    rdfs:label "Division - D144 Division 4 Exports of sheep by sea to the Middle East"@en-AU ;
    dct:hasPart F2021L00319:145,
        F2021L00319:147,
        F2021L00319:148,
        F2021L00319:149,
        F2021L00319:150,
        F2021L00319:151,
        F2021L00319:152,
        F2021L00319:153,
        F2021L00319:154,
        F2021L00319:155,
        F2021L00319:156,
        F2021L00319:157,
        F2021L00319:158,
        F2021L00319:159,
        F2021L00319:160,
        F2021L00319:161,
        F2021L00319:162,
        F2021L00319:163,
        F2021L00319:164 ;
    dct:isPartOf F2021L00319:132 ;
    dct:isReferencedBy F2021L00319: ;
    rdfs:comment "Division 4 Exports of sheep by sea to the Middle East - Abrievated Graph Key: D144"@en-AU ;
    skos:broader F2021L00319:145,
        F2021L00319:147,
        F2021L00319:148,
        F2021L00319:149,
        F2021L00319:150,
        F2021L00319:151,
        F2021L00319:152,
        F2021L00319:153,
        F2021L00319:154,
        F2021L00319:155,
        F2021L00319:156,
        F2021L00319:157,
        F2021L00319:158,
        F2021L00319:159,
        F2021L00319:160,
        F2021L00319:161,
        F2021L00319:162,
        F2021L00319:163,
        F2021L00319:164 ;
    skos:definition "Division 4 Exports of sheep by sea to the Middle East"@en-AU ;
    skos:narrower F2021L00319:132 ;
    skos:prefLabel "Division D144"@en-AU ;
    dcat:accessURL <https://www.legislation.gov.au/F2021L00319/2024-04-30/2024-04-30/text/original/epub/OEBPS/document_1/document_1.html#_Toc166157977> ;
    dcat:landingPage "https://www.legislation.gov.au/F2021L00319/2024-04-30/2024-04-30/text/original/epub/OEBPS/document_1/document_1.html#_Toc166157977"^^xsd:anyURI ;
    dcat:theme legcons:Division .

F2021L00319:125 a legcons:Chapter,
        owl:Class,
        dcat:Resource ;
    rdfs:label "Chapter - C125 Chapter 6 Livestock export licences"@en-AU ;
    dct:hasPart F2021L00319:126,
        F2021L00319:132,
        F2021L00319:168,
        F2021L00319:169,
        F2021L00319:170,
        F2021L00319:171,
        F2021L00319:172,
        F2021L00319:173,
        F2021L00319:174,
        F2021L00319:175,
        F2021L00319:176,
        F2021L00319:177,
        F2021L00319:178,
        F2021L00319:179,
        F2021L00319:180,
        F2021L00319:181,
        F2021L00319:182,
        F2021L00319:183,
        F2021L00319:189,
        F2021L00319:193,
        F2021L00319:196,
        F2021L00319:198,
        F2021L00319:199 ;
    dct:isReferencedBy F2021L00319: ;
    rdfs:comment "Chapter 6 Livestock export licences - Abrievated Graph Key: C125"@en-AU ;
    skos:broader F2021L00319:126,
        F2021L00319:132,
        F2021L00319:168,
        F2021L00319:169,
        F2021L00319:170,
        F2021L00319:171,
        F2021L00319:172,
        F2021L00319:173,
        F2021L00319:174,
        F2021L00319:175,
        F2021L00319:176,
        F2021L00319:177,
        F2021L00319:178,
        F2021L00319:179,
        F2021L00319:180,
        F2021L00319:181,
        F2021L00319:182,
        F2021L00319:183,
        F2021L00319:189,
        F2021L00319:193,
        F2021L00319:196,
        F2021L00319:198,
        F2021L00319:199 ;
    skos:definition "Chapter 6 Livestock export licences"@en-AU ;
    skos:prefLabel "Chapter C125"@en-AU ;
    dcat:accessURL <https://www.legislation.gov.au/F2021L00319/2024-04-30/2024-04-30/text/original/epub/OEBPS/document_1/document_1.html#_Toc166157958> ;
    dcat:landingPage "https://www.legislation.gov.au/F2021L00319/2024-04-30/2024-04-30/text/original/epub/OEBPS/document_1/document_1.html#_Toc166157958"^^xsd:anyURI ;
    dcat:theme legcons:Chapter .

F2021L00319: a owl:Class,
        dcat:Dataset,
        dcat:Resource ;
    rdfs:label "Export Control (Animals) Rules 2021" ;
    dct:Jurisdiction " Department of Agriculture, Fisheries and Forestry "@en-AU ;
    dct:created "2024-08-30T15:10:08.657147"^^xsd:dateTime ;
    dct:creator "https://orcid.org/0009-0007-8434-7325"^^xsd:anyURI ;
    dct:date "2024-04-30T00:00:00+10:00"^^xsd:dateTime ;
    dct:description "Export Control (Animals) Rules 2021"@en-AU ;
    dct:identifier "https://www.legislation.gov.au/F2021L00319/latest"^^xsd:anyURI ;
    dct:license <https://creativecommons.org/licenses/by-sa/4.0/> ;
    dct:source "scheme=AGLSTERMS.AglsAgent; corporateName=Office Parliamentary Counsel; address=Locked Bag 30 Kingston ACT 2604; contact=+61 2 6120 1400"@en-AU ;
    dct:subject "Export Control (Animals) Rules 2021"@en-AU ;
    dct:title "Export Control (Animals) Rules 2021"@en-AU ;
    owl:imports legcons: ;
    dcat:theme legcons:Chapter,
        legcons:Division,
        legcons:Endnotes,
        legcons:Item,
        legcons:Part,
        legcons:Subdivision ;
    schema:identifier "F2021L00319" ;
    schema:status "In force" ;
    schema:version "F2024C00422 (C06)" .

