@prefix F2021L00308: <http://example.org/au/leg/dataset/F2021L00308/> .
@prefix dcat: <http://www.w3.org/ns/dcat#> .
@prefix dct: <http://purl.org/dc/terms/> .
@prefix legcons: <http://example.org/au/leg/concepts/> .
@prefix owl: <http://www.w3.org/2002/07/owl#> .
@prefix rdfs: <http://www.w3.org/2000/01/rdf-schema#> .
@prefix schema: <https://schema.org/> .
@prefix skos: <http://www.w3.org/2004/02/skos/core#> .
@prefix xsd: <http://www.w3.org/2001/XMLSchema#> .

F2021L00308:10 a legcons:Division,
        owl:Class,
        dcat:Resource ;
    rdfs:label "Division - D10 Division 2 Other interpretation provisions"@en-AU ;
    dct:isPartOf F2021L00308:1 ;
    dct:isReferencedBy F2021L00308: ;
    rdfs:comment "Division 2 Other interpretation provisions - Abrievated Graph Key: D10"@en-AU ;
    skos:definition "Division 2 Other interpretation provisions"@en-AU ;
    skos:narrower F2021L00308:1 ;
    skos:prefLabel "Division D10"@en-AU ;
    dcat:accessURL <https://www.legislation.gov.au/F2021L00308/2023-08-04/2023-08-04/text/original/epub/OEBPS/document_1/document_1.html#_Toc143604719> ;
    dcat:landingPage "https://www.legislation.gov.au/F2021L00308/2023-08-04/2023-08-04/text/original/epub/OEBPS/document_1/document_1.html#_Toc143604719"^^xsd:anyURI ;
    dcat:theme legcons:Division .

F2021L00308:100 a legcons:Item,
        owl:Class,
        dcat:Resource ;
    rdfs:label "Item - I100 5 12  Dressing ratites"@en-AU ;
    dct:isPartOf F2021L00308:90 ;
    dct:isReferencedBy F2021L00308: ;
    rdfs:comment "5 12  Dressing ratites - Abrievated Graph Key: I100"@en-AU ;
    skos:definition "5 12  Dressing ratites"@en-AU ;
    skos:narrower F2021L00308:90 ;
    skos:prefLabel "Item I100"@en-AU ;
    dcat:accessURL <https://www.legislation.gov.au/F2021L00308/2023-08-04/2023-08-04/text/original/epub/OEBPS/document_1/document_1.html#_Toc143604809> ;
    dcat:landingPage "https://www.legislation.gov.au/F2021L00308/2023-08-04/2023-08-04/text/original/epub/OEBPS/document_1/document_1.html#_Toc143604809"^^xsd:anyURI ;
    dcat:theme legcons:Item .

F2021L00308:101 a legcons:Item,
        owl:Class,
        dcat:Resource ;
    rdfs:label "Item - I101 5 13  Chilling ratite carcases"@en-AU ;
    dct:isPartOf F2021L00308:90 ;
    dct:isReferencedBy F2021L00308: ;
    rdfs:comment "5 13  Chilling ratite carcases - Abrievated Graph Key: I101"@en-AU ;
    skos:definition "5 13  Chilling ratite carcases"@en-AU ;
    skos:narrower F2021L00308:90 ;
    skos:prefLabel "Item I101"@en-AU ;
    dcat:accessURL <https://www.legislation.gov.au/F2021L00308/2023-08-04/2023-08-04/text/original/epub/OEBPS/document_1/document_1.html#_Toc143604810> ;
    dcat:landingPage "https://www.legislation.gov.au/F2021L00308/2023-08-04/2023-08-04/text/original/epub/OEBPS/document_1/document_1.html#_Toc143604810"^^xsd:anyURI ;
    dcat:theme legcons:Item .

F2021L00308:102 a legcons:Item,
        owl:Class,
        dcat:Resource ;
    rdfs:label "Item - I102 5 14  Removal of microchips from prescribed ratite meat and ratite meat products"@en-AU ;
    dct:isPartOf F2021L00308:90 ;
    dct:isReferencedBy F2021L00308: ;
    rdfs:comment "5 14  Removal of microchips from prescribed ratite meat and ratite meat products - Abrievated Graph Key: I102"@en-AU ;
    skos:definition "5 14  Removal of microchips from prescribed ratite meat and ratite meat products"@en-AU ;
    skos:narrower F2021L00308:90 ;
    skos:prefLabel "Item I102"@en-AU ;
    dcat:accessURL <https://www.legislation.gov.au/F2021L00308/2023-08-04/2023-08-04/text/original/epub/OEBPS/document_1/document_1.html#_Toc143604811> ;
    dcat:landingPage "https://www.legislation.gov.au/F2021L00308/2023-08-04/2023-08-04/text/original/epub/OEBPS/document_1/document_1.html#_Toc143604811"^^xsd:anyURI ;
    dcat:theme legcons:Item .

F2021L00308:103 a legcons:Item,
        owl:Class,
        dcat:Resource ;
    rdfs:label "Item - I103 5 15  Ratite fat"@en-AU ;
    dct:isPartOf F2021L00308:90 ;
    dct:isReferencedBy F2021L00308: ;
    rdfs:comment "5 15  Ratite fat - Abrievated Graph Key: I103"@en-AU ;
    skos:definition "5 15  Ratite fat"@en-AU ;
    skos:narrower F2021L00308:90 ;
    skos:prefLabel "Item I103"@en-AU ;
    dcat:accessURL <https://www.legislation.gov.au/F2021L00308/2023-08-04/2023-08-04/text/original/epub/OEBPS/document_1/document_1.html#_Toc143604812> ;
    dcat:landingPage "https://www.legislation.gov.au/F2021L00308/2023-08-04/2023-08-04/text/original/epub/OEBPS/document_1/document_1.html#_Toc143604812"^^xsd:anyURI ;
    dcat:theme legcons:Item .

F2021L00308:104 a legcons:Division,
        owl:Class,
        dcat:Resource ;
    rdfs:label "Division - D104 Division 4 Transport"@en-AU ;
    dct:isPartOf F2021L00308:84 ;
    dct:isReferencedBy F2021L00308: ;
    rdfs:comment "Division 4 Transport - Abrievated Graph Key: D104"@en-AU ;
    skos:definition "Division 4 Transport"@en-AU ;
    skos:narrower F2021L00308:84 ;
    skos:prefLabel "Division D104"@en-AU ;
    dcat:accessURL <https://www.legislation.gov.au/F2021L00308/2023-08-04/2023-08-04/text/original/epub/OEBPS/document_1/document_1.html#_Toc143604813> ;
    dcat:landingPage "https://www.legislation.gov.au/F2021L00308/2023-08-04/2023-08-04/text/original/epub/OEBPS/document_1/document_1.html#_Toc143604813"^^xsd:anyURI ;
    dcat:theme legcons:Division .

F2021L00308:105 a legcons:Item,
        owl:Class,
        dcat:Resource ;
    rdfs:label "Item - I105 5 16  Loading prescribed rabbit meat ratite meat rabbit meat products or ratite meat products for transfer between registered establishments"@en-AU ;
    dct:isPartOf F2021L00308:84 ;
    dct:isReferencedBy F2021L00308: ;
    rdfs:comment "5 16  Loading prescribed rabbit meat ratite meat rabbit meat products or ratite meat products for transfer between registered establishments - Abrievated Graph Key: I105"@en-AU ;
    skos:definition "5 16  Loading prescribed rabbit meat ratite meat rabbit meat products or ratite meat products for transfer between registered establishments"@en-AU ;
    skos:narrower F2021L00308:84 ;
    skos:prefLabel "Item I105"@en-AU ;
    dcat:accessURL <https://www.legislation.gov.au/F2021L00308/2023-08-04/2023-08-04/text/original/epub/OEBPS/document_1/document_1.html#_Toc143604814> ;
    dcat:landingPage "https://www.legislation.gov.au/F2021L00308/2023-08-04/2023-08-04/text/original/epub/OEBPS/document_1/document_1.html#_Toc143604814"^^xsd:anyURI ;
    dcat:theme legcons:Item .

F2021L00308:106 a legcons:Item,
        owl:Class,
        dcat:Resource ;
    rdfs:label "Item - I106 5 17  Loading of prescribed rabbit meat ratite meat rabbit meat products or ratite meat productssupervision"@en-AU ;
    dct:isPartOf F2021L00308:84 ;
    dct:isReferencedBy F2021L00308: ;
    rdfs:comment "5 17  Loading of prescribed rabbit meat ratite meat rabbit meat products or ratite meat productssupervision - Abrievated Graph Key: I106"@en-AU ;
    skos:definition "5 17  Loading of prescribed rabbit meat ratite meat rabbit meat products or ratite meat productssupervision"@en-AU ;
    skos:narrower F2021L00308:84 ;
    skos:prefLabel "Item I106"@en-AU ;
    dcat:accessURL <https://www.legislation.gov.au/F2021L00308/2023-08-04/2023-08-04/text/original/epub/OEBPS/document_1/document_1.html#_Toc143604815> ;
    dcat:landingPage "https://www.legislation.gov.au/F2021L00308/2023-08-04/2023-08-04/text/original/epub/OEBPS/document_1/document_1.html#_Toc143604815"^^xsd:anyURI ;
    dcat:theme legcons:Item .

F2021L00308:107 a legcons:Item,
        owl:Class,
        dcat:Resource ;
    rdfs:label "Item - I107 5 18  Prohibitions on loading"@en-AU ;
    dct:isPartOf F2021L00308:84 ;
    dct:isReferencedBy F2021L00308: ;
    rdfs:comment "5 18  Prohibitions on loading - Abrievated Graph Key: I107"@en-AU ;
    skos:definition "5 18  Prohibitions on loading"@en-AU ;
    skos:narrower F2021L00308:84 ;
    skos:prefLabel "Item I107"@en-AU ;
    dcat:accessURL <https://www.legislation.gov.au/F2021L00308/2023-08-04/2023-08-04/text/original/epub/OEBPS/document_1/document_1.html#_Toc143604816> ;
    dcat:landingPage "https://www.legislation.gov.au/F2021L00308/2023-08-04/2023-08-04/text/original/epub/OEBPS/document_1/document_1.html#_Toc143604816"^^xsd:anyURI ;
    dcat:theme legcons:Item .

F2021L00308:108 a legcons:Item,
        owl:Class,
        dcat:Resource ;
    rdfs:label "Item - I108 5 19  Container system units and equipment for loading aircraft and vessels"@en-AU ;
    dct:isPartOf F2021L00308:84 ;
    dct:isReferencedBy F2021L00308: ;
    rdfs:comment "5 19  Container system units and equipment for loading aircraft and vessels - Abrievated Graph Key: I108"@en-AU ;
    skos:definition "5 19  Container system units and equipment for loading aircraft and vessels"@en-AU ;
    skos:narrower F2021L00308:84 ;
    skos:prefLabel "Item I108"@en-AU ;
    dcat:accessURL <https://www.legislation.gov.au/F2021L00308/2023-08-04/2023-08-04/text/original/epub/OEBPS/document_1/document_1.html#_Toc143604817> ;
    dcat:landingPage "https://www.legislation.gov.au/F2021L00308/2023-08-04/2023-08-04/text/original/epub/OEBPS/document_1/document_1.html#_Toc143604817"^^xsd:anyURI ;
    dcat:theme legcons:Item .

F2021L00308:109 a legcons:Item,
        owl:Class,
        dcat:Resource ;
    rdfs:label "Item - I109 5 20  When a bolt seal must be applied to container system unit"@en-AU ;
    dct:isPartOf F2021L00308:84 ;
    dct:isReferencedBy F2021L00308: ;
    rdfs:comment "5 20  When a bolt seal must be applied to container system unit - Abrievated Graph Key: I109"@en-AU ;
    skos:definition "5 20  When a bolt seal must be applied to container system unit"@en-AU ;
    skos:narrower F2021L00308:84 ;
    skos:prefLabel "Item I109"@en-AU ;
    dcat:accessURL <https://www.legislation.gov.au/F2021L00308/2023-08-04/2023-08-04/text/original/epub/OEBPS/document_1/document_1.html#_Toc143604818> ;
    dcat:landingPage "https://www.legislation.gov.au/F2021L00308/2023-08-04/2023-08-04/text/original/epub/OEBPS/document_1/document_1.html#_Toc143604818"^^xsd:anyURI ;
    dcat:theme legcons:Item .

F2021L00308:11 a legcons:Item,
        owl:Class,
        dcat:Resource ;
    rdfs:label "Item - I11 1 7  References to authorised officer and meat safety inspector"@en-AU ;
    dct:isPartOf F2021L00308:1 ;
    dct:isReferencedBy F2021L00308: ;
    rdfs:comment "1 7  References to authorised officer and meat safety inspector - Abrievated Graph Key: I11"@en-AU ;
    skos:definition "1 7  References to authorised officer and meat safety inspector"@en-AU ;
    skos:narrower F2021L00308:1 ;
    skos:prefLabel "Item I11"@en-AU ;
    dcat:accessURL <https://www.legislation.gov.au/F2021L00308/2023-08-04/2023-08-04/text/original/epub/OEBPS/document_1/document_1.html#_Toc143604720> ;
    dcat:landingPage "https://www.legislation.gov.au/F2021L00308/2023-08-04/2023-08-04/text/original/epub/OEBPS/document_1/document_1.html#_Toc143604720"^^xsd:anyURI ;
    dcat:theme legcons:Item .

F2021L00308:110 a legcons:Item,
        owl:Class,
        dcat:Resource ;
    rdfs:label "Item - I110 5 21  Meat transport vehicles measuring devices and other equipment"@en-AU ;
    dct:isPartOf F2021L00308:84 ;
    dct:isReferencedBy F2021L00308: ;
    rdfs:comment "5 21  Meat transport vehicles measuring devices and other equipment - Abrievated Graph Key: I110"@en-AU ;
    skos:definition "5 21  Meat transport vehicles measuring devices and other equipment"@en-AU ;
    skos:narrower F2021L00308:84 ;
    skos:prefLabel "Item I110"@en-AU ;
    dcat:accessURL <https://www.legislation.gov.au/F2021L00308/2023-08-04/2023-08-04/text/original/epub/OEBPS/document_1/document_1.html#_Toc143604819> ;
    dcat:landingPage "https://www.legislation.gov.au/F2021L00308/2023-08-04/2023-08-04/text/original/epub/OEBPS/document_1/document_1.html#_Toc143604819"^^xsd:anyURI ;
    dcat:theme legcons:Item .

F2021L00308:111 a legcons:Division,
        owl:Class,
        dcat:Resource ;
    rdfs:label "Division - D111 Division 5 Trade descriptions"@en-AU ;
    dct:isPartOf F2021L00308:84 ;
    dct:isReferencedBy F2021L00308: ;
    rdfs:comment "Division 5 Trade descriptions - Abrievated Graph Key: D111"@en-AU ;
    skos:definition "Division 5 Trade descriptions"@en-AU ;
    skos:narrower F2021L00308:84 ;
    skos:prefLabel "Division D111"@en-AU ;
    dcat:accessURL <https://www.legislation.gov.au/F2021L00308/2023-08-04/2023-08-04/text/original/epub/OEBPS/document_1/document_1.html#_Toc143604820> ;
    dcat:landingPage "https://www.legislation.gov.au/F2021L00308/2023-08-04/2023-08-04/text/original/epub/OEBPS/document_1/document_1.html#_Toc143604820"^^xsd:anyURI ;
    dcat:theme legcons:Division .

F2021L00308:113 a legcons:Item,
        owl:Class,
        dcat:Resource ;
    rdfs:label "Item - I113 5 22  Trade description must be applied to prescribed rabbit meat ratite meat rabbit meat products and ratite meat products that are intended to be exported"@en-AU ;
    dct:isPartOf F2021L00308:112 ;
    dct:isReferencedBy F2021L00308: ;
    rdfs:comment "5 22  Trade description must be applied to prescribed rabbit meat ratite meat rabbit meat products and ratite meat products that are intended to be exported - Abrievated Graph Key: I113"@en-AU ;
    skos:definition "5 22  Trade description must be applied to prescribed rabbit meat ratite meat rabbit meat products and ratite meat products that are intended to be exported"@en-AU ;
    skos:narrower F2021L00308:112 ;
    skos:prefLabel "Item I113"@en-AU ;
    dcat:accessURL <https://www.legislation.gov.au/F2021L00308/2023-08-04/2023-08-04/text/original/epub/OEBPS/document_1/document_1.html#_Toc143604822> ;
    dcat:landingPage "https://www.legislation.gov.au/F2021L00308/2023-08-04/2023-08-04/text/original/epub/OEBPS/document_1/document_1.html#_Toc143604822"^^xsd:anyURI ;
    dcat:theme legcons:Item .

F2021L00308:114 a legcons:Item,
        owl:Class,
        dcat:Resource ;
    rdfs:label "Item - I114 5 23  Prescribed rabbit meat ratite meat rabbit meat products or ratite meat products in cartons or cans"@en-AU ;
    dct:isPartOf F2021L00308:112 ;
    dct:isReferencedBy F2021L00308: ;
    rdfs:comment "5 23  Prescribed rabbit meat ratite meat rabbit meat products or ratite meat products in cartons or cans - Abrievated Graph Key: I114"@en-AU ;
    skos:definition "5 23  Prescribed rabbit meat ratite meat rabbit meat products or ratite meat products in cartons or cans"@en-AU ;
    skos:narrower F2021L00308:112 ;
    skos:prefLabel "Item I114"@en-AU ;
    dcat:accessURL <https://www.legislation.gov.au/F2021L00308/2023-08-04/2023-08-04/text/original/epub/OEBPS/document_1/document_1.html#_Toc143604823> ;
    dcat:landingPage "https://www.legislation.gov.au/F2021L00308/2023-08-04/2023-08-04/text/original/epub/OEBPS/document_1/document_1.html#_Toc143604823"^^xsd:anyURI ;
    dcat:theme legcons:Item .

F2021L00308:115 a legcons:Item,
        owl:Class,
        dcat:Resource ;
    rdfs:label "Item - I115 5 24  Prescribed rabbit meat ratite meat rabbit meat products or ratite meat products for further processing"@en-AU ;
    dct:isPartOf F2021L00308:112 ;
    dct:isReferencedBy F2021L00308: ;
    rdfs:comment "5 24  Prescribed rabbit meat ratite meat rabbit meat products or ratite meat products for further processing - Abrievated Graph Key: I115"@en-AU ;
    skos:definition "5 24  Prescribed rabbit meat ratite meat rabbit meat products or ratite meat products for further processing"@en-AU ;
    skos:narrower F2021L00308:112 ;
    skos:prefLabel "Item I115"@en-AU ;
    dcat:accessURL <https://www.legislation.gov.au/F2021L00308/2023-08-04/2023-08-04/text/original/epub/OEBPS/document_1/document_1.html#_Toc143604824> ;
    dcat:landingPage "https://www.legislation.gov.au/F2021L00308/2023-08-04/2023-08-04/text/original/epub/OEBPS/document_1/document_1.html#_Toc143604824"^^xsd:anyURI ;
    dcat:theme legcons:Item .

F2021L00308:117 a legcons:Item,
        owl:Class,
        dcat:Resource ;
    rdfs:label "Item - I117 5 25  Application of this Subdivision"@en-AU ;
    dct:isPartOf F2021L00308:116 ;
    dct:isReferencedBy F2021L00308: ;
    rdfs:comment "5 25  Application of this Subdivision - Abrievated Graph Key: I117"@en-AU ;
    skos:definition "5 25  Application of this Subdivision"@en-AU ;
    skos:narrower F2021L00308:116 ;
    skos:prefLabel "Item I117"@en-AU ;
    dcat:accessURL <https://www.legislation.gov.au/F2021L00308/2023-08-04/2023-08-04/text/original/epub/OEBPS/document_1/document_1.html#_Toc143604826> ;
    dcat:landingPage "https://www.legislation.gov.au/F2021L00308/2023-08-04/2023-08-04/text/original/epub/OEBPS/document_1/document_1.html#_Toc143604826"^^xsd:anyURI ;
    dcat:theme legcons:Item .

F2021L00308:118 a legcons:Item,
        owl:Class,
        dcat:Resource ;
    rdfs:label "Item - I118 5 26  Trade descriptions applied to rabbit carcases"@en-AU ;
    dct:isPartOf F2021L00308:116 ;
    dct:isReferencedBy F2021L00308: ;
    rdfs:comment "5 26  Trade descriptions applied to rabbit carcases - Abrievated Graph Key: I118"@en-AU ;
    skos:definition "5 26  Trade descriptions applied to rabbit carcases"@en-AU ;
    skos:narrower F2021L00308:116 ;
    skos:prefLabel "Item I118"@en-AU ;
    dcat:accessURL <https://www.legislation.gov.au/F2021L00308/2023-08-04/2023-08-04/text/original/epub/OEBPS/document_1/document_1.html#_Toc143604827> ;
    dcat:landingPage "https://www.legislation.gov.au/F2021L00308/2023-08-04/2023-08-04/text/original/epub/OEBPS/document_1/document_1.html#_Toc143604827"^^xsd:anyURI ;
    dcat:theme legcons:Item .

F2021L00308:119 a legcons:Item,
        owl:Class,
        dcat:Resource ;
    rdfs:label "Item - I119 5 27  Trade description applied to rabbit carcase parts"@en-AU ;
    dct:isPartOf F2021L00308:116 ;
    dct:isReferencedBy F2021L00308: ;
    rdfs:comment "5 27  Trade description applied to rabbit carcase parts - Abrievated Graph Key: I119"@en-AU ;
    skos:definition "5 27  Trade description applied to rabbit carcase parts"@en-AU ;
    skos:narrower F2021L00308:116 ;
    skos:prefLabel "Item I119"@en-AU ;
    dcat:accessURL <https://www.legislation.gov.au/F2021L00308/2023-08-04/2023-08-04/text/original/epub/OEBPS/document_1/document_1.html#_Toc143604828> ;
    dcat:landingPage "https://www.legislation.gov.au/F2021L00308/2023-08-04/2023-08-04/text/original/epub/OEBPS/document_1/document_1.html#_Toc143604828"^^xsd:anyURI ;
    dcat:theme legcons:Item .

F2021L00308:12 a legcons:Item,
        owl:Class,
        dcat:Resource ;
    rdfs:label "Item - I12 1 8  Modifications of certain terms used in the Australian Meat Standard"@en-AU ;
    dct:isPartOf F2021L00308:1 ;
    dct:isReferencedBy F2021L00308: ;
    rdfs:comment "1 8  Modifications of certain terms used in the Australian Meat Standard - Abrievated Graph Key: I12"@en-AU ;
    skos:definition "1 8  Modifications of certain terms used in the Australian Meat Standard"@en-AU ;
    skos:narrower F2021L00308:1 ;
    skos:prefLabel "Item I12"@en-AU ;
    dcat:accessURL <https://www.legislation.gov.au/F2021L00308/2023-08-04/2023-08-04/text/original/epub/OEBPS/document_1/document_1.html#_Toc143604721> ;
    dcat:landingPage "https://www.legislation.gov.au/F2021L00308/2023-08-04/2023-08-04/text/original/epub/OEBPS/document_1/document_1.html#_Toc143604721"^^xsd:anyURI ;
    dcat:theme legcons:Item .

F2021L00308:120 a legcons:Division,
        owl:Class,
        dcat:Resource ;
    rdfs:label "Division - D120 Division 6 Official marks"@en-AU ;
    dct:isPartOf F2021L00308:84 ;
    dct:isReferencedBy F2021L00308: ;
    rdfs:comment "Division 6 Official marks - Abrievated Graph Key: D120"@en-AU ;
    skos:definition "Division 6 Official marks"@en-AU ;
    skos:narrower F2021L00308:84 ;
    skos:prefLabel "Division D120"@en-AU ;
    dcat:accessURL <https://www.legislation.gov.au/F2021L00308/2023-08-04/2023-08-04/text/original/epub/OEBPS/document_1/document_1.html#_Toc143604829> ;
    dcat:landingPage "https://www.legislation.gov.au/F2021L00308/2023-08-04/2023-08-04/text/original/epub/OEBPS/document_1/document_1.html#_Toc143604829"^^xsd:anyURI ;
    dcat:theme legcons:Division .

F2021L00308:121 a legcons:Item,
        owl:Class,
        dcat:Resource ;
    rdfs:label "Item - I121 5 28  References to particular official marks"@en-AU ;
    dct:isPartOf F2021L00308:84 ;
    dct:isReferencedBy F2021L00308: ;
    rdfs:comment "5 28  References to particular official marks - Abrievated Graph Key: I121"@en-AU ;
    skos:definition "5 28  References to particular official marks"@en-AU ;
    skos:narrower F2021L00308:84 ;
    skos:prefLabel "Item I121"@en-AU ;
    dcat:accessURL <https://www.legislation.gov.au/F2021L00308/2023-08-04/2023-08-04/text/original/epub/OEBPS/document_1/document_1.html#_Toc143604830> ;
    dcat:landingPage "https://www.legislation.gov.au/F2021L00308/2023-08-04/2023-08-04/text/original/epub/OEBPS/document_1/document_1.html#_Toc143604830"^^xsd:anyURI ;
    dcat:theme legcons:Item .

F2021L00308:122 a legcons:Item,
        owl:Class,
        dcat:Resource ;
    rdfs:label "Item - I122 5 29  Carcases and carcase parts"@en-AU ;
    dct:isPartOf F2021L00308:84 ;
    dct:isReferencedBy F2021L00308: ;
    rdfs:comment "5 29  Carcases and carcase parts - Abrievated Graph Key: I122"@en-AU ;
    skos:definition "5 29  Carcases and carcase parts"@en-AU ;
    skos:narrower F2021L00308:84 ;
    skos:prefLabel "Item I122"@en-AU ;
    dcat:accessURL <https://www.legislation.gov.au/F2021L00308/2023-08-04/2023-08-04/text/original/epub/OEBPS/document_1/document_1.html#_Toc143604831> ;
    dcat:landingPage "https://www.legislation.gov.au/F2021L00308/2023-08-04/2023-08-04/text/original/epub/OEBPS/document_1/document_1.html#_Toc143604831"^^xsd:anyURI ;
    dcat:theme legcons:Item .

F2021L00308:123 a legcons:Item,
        owl:Class,
        dcat:Resource ;
    rdfs:label "Item - I123 5 30  Cartons containing prescribed rabbit meat ratite meat rabbit meat products or ratite meat products"@en-AU ;
    dct:isPartOf F2021L00308:84 ;
    dct:isReferencedBy F2021L00308: ;
    rdfs:comment "5 30  Cartons containing prescribed rabbit meat ratite meat rabbit meat products or ratite meat products - Abrievated Graph Key: I123"@en-AU ;
    skos:definition "5 30  Cartons containing prescribed rabbit meat ratite meat rabbit meat products or ratite meat products"@en-AU ;
    skos:narrower F2021L00308:84 ;
    skos:prefLabel "Item I123"@en-AU ;
    dcat:accessURL <https://www.legislation.gov.au/F2021L00308/2023-08-04/2023-08-04/text/original/epub/OEBPS/document_1/document_1.html#_Toc143604832> ;
    dcat:landingPage "https://www.legislation.gov.au/F2021L00308/2023-08-04/2023-08-04/text/original/epub/OEBPS/document_1/document_1.html#_Toc143604832"^^xsd:anyURI ;
    dcat:theme legcons:Item .

F2021L00308:124 a legcons:Item,
        owl:Class,
        dcat:Resource ;
    rdfs:label "Item - I124 5 31  State or Territory classification marks must not be applied"@en-AU ;
    dct:isPartOf F2021L00308:84 ;
    dct:isReferencedBy F2021L00308: ;
    rdfs:comment "5 31  State or Territory classification marks must not be applied - Abrievated Graph Key: I124"@en-AU ;
    skos:definition "5 31  State or Territory classification marks must not be applied"@en-AU ;
    skos:narrower F2021L00308:84 ;
    skos:prefLabel "Item I124"@en-AU ;
    dcat:accessURL <https://www.legislation.gov.au/F2021L00308/2023-08-04/2023-08-04/text/original/epub/OEBPS/document_1/document_1.html#_Toc143604833> ;
    dcat:landingPage "https://www.legislation.gov.au/F2021L00308/2023-08-04/2023-08-04/text/original/epub/OEBPS/document_1/document_1.html#_Toc143604833"^^xsd:anyURI ;
    dcat:theme legcons:Item .

F2021L00308:125 a legcons:Division,
        owl:Class,
        dcat:Resource ;
    rdfs:label "Division - D125 Division 7 Segregation identification security traceability and integrity"@en-AU ;
    dct:isPartOf F2021L00308:84 ;
    dct:isReferencedBy F2021L00308: ;
    rdfs:comment "Division 7 Segregation identification security traceability and integrity - Abrievated Graph Key: D125"@en-AU ;
    skos:definition "Division 7 Segregation identification security traceability and integrity"@en-AU ;
    skos:narrower F2021L00308:84 ;
    skos:prefLabel "Division D125"@en-AU ;
    dcat:accessURL <https://www.legislation.gov.au/F2021L00308/2023-08-04/2023-08-04/text/original/epub/OEBPS/document_1/document_1.html#_Toc143604834> ;
    dcat:landingPage "https://www.legislation.gov.au/F2021L00308/2023-08-04/2023-08-04/text/original/epub/OEBPS/document_1/document_1.html#_Toc143604834"^^xsd:anyURI ;
    dcat:theme legcons:Division .

F2021L00308:126 a legcons:Item,
        owl:Class,
        dcat:Resource ;
    rdfs:label "Item - I126 5 32  Segregation identification security and traceabilitygeneral"@en-AU ;
    dct:isPartOf F2021L00308:84 ;
    dct:isReferencedBy F2021L00308: ;
    rdfs:comment "5 32  Segregation identification security and traceabilitygeneral - Abrievated Graph Key: I126"@en-AU ;
    skos:definition "5 32  Segregation identification security and traceabilitygeneral"@en-AU ;
    skos:narrower F2021L00308:84 ;
    skos:prefLabel "Item I126"@en-AU ;
    dcat:accessURL <https://www.legislation.gov.au/F2021L00308/2023-08-04/2023-08-04/text/original/epub/OEBPS/document_1/document_1.html#_Toc143604835> ;
    dcat:landingPage "https://www.legislation.gov.au/F2021L00308/2023-08-04/2023-08-04/text/original/epub/OEBPS/document_1/document_1.html#_Toc143604835"^^xsd:anyURI ;
    dcat:theme legcons:Item .

F2021L00308:127 a legcons:Item,
        owl:Class,
        dcat:Resource ;
    rdfs:label "Item - I127 5 33  Establishments where rabbit meat ratite meat rabbit meat products or ratite meat products that are not for export etc are prepared"@en-AU ;
    dct:isPartOf F2021L00308:84 ;
    dct:isReferencedBy F2021L00308: ;
    rdfs:comment "5 33  Establishments where rabbit meat ratite meat rabbit meat products or ratite meat products that are not for export etc are prepared - Abrievated Graph Key: I127"@en-AU ;
    skos:definition "5 33  Establishments where rabbit meat ratite meat rabbit meat products or ratite meat products that are not for export etc are prepared"@en-AU ;
    skos:narrower F2021L00308:84 ;
    skos:prefLabel "Item I127"@en-AU ;
    dcat:accessURL <https://www.legislation.gov.au/F2021L00308/2023-08-04/2023-08-04/text/original/epub/OEBPS/document_1/document_1.html#_Toc143604836> ;
    dcat:landingPage "https://www.legislation.gov.au/F2021L00308/2023-08-04/2023-08-04/text/original/epub/OEBPS/document_1/document_1.html#_Toc143604836"^^xsd:anyURI ;
    dcat:theme legcons:Item .

F2021L00308:128 a legcons:Item,
        owl:Class,
        dcat:Resource ;
    rdfs:label "Item - I128 5 34  Integritygeneral"@en-AU ;
    dct:isPartOf F2021L00308:84 ;
    dct:isReferencedBy F2021L00308: ;
    rdfs:comment "5 34  Integritygeneral - Abrievated Graph Key: I128"@en-AU ;
    skos:definition "5 34  Integritygeneral"@en-AU ;
    skos:narrower F2021L00308:84 ;
    skos:prefLabel "Item I128"@en-AU ;
    dcat:accessURL <https://www.legislation.gov.au/F2021L00308/2023-08-04/2023-08-04/text/original/epub/OEBPS/document_1/document_1.html#_Toc143604837> ;
    dcat:landingPage "https://www.legislation.gov.au/F2021L00308/2023-08-04/2023-08-04/text/original/epub/OEBPS/document_1/document_1.html#_Toc143604837"^^xsd:anyURI ;
    dcat:theme legcons:Item .

F2021L00308:129 a legcons:Item,
        owl:Class,
        dcat:Resource ;
    rdfs:label "Item - I129 5 35  Identificationtype of animal"@en-AU ;
    dct:isPartOf F2021L00308:84 ;
    dct:isReferencedBy F2021L00308: ;
    rdfs:comment "5 35  Identificationtype of animal - Abrievated Graph Key: I129"@en-AU ;
    skos:definition "5 35  Identificationtype of animal"@en-AU ;
    skos:narrower F2021L00308:84 ;
    skos:prefLabel "Item I129"@en-AU ;
    dcat:accessURL <https://www.legislation.gov.au/F2021L00308/2023-08-04/2023-08-04/text/original/epub/OEBPS/document_1/document_1.html#_Toc143604838> ;
    dcat:landingPage "https://www.legislation.gov.au/F2021L00308/2023-08-04/2023-08-04/text/original/epub/OEBPS/document_1/document_1.html#_Toc143604838"^^xsd:anyURI ;
    dcat:theme legcons:Item .

F2021L00308:13 a legcons:Item,
        owl:Class,
        dcat:Resource ;
    rdfs:label "Item - I13 1 9  Circumstances in which alternative procedure standard or other requirement is taken to meet requirements of Australian Meat Standard"@en-AU ;
    dct:isPartOf F2021L00308:1 ;
    dct:isReferencedBy F2021L00308: ;
    rdfs:comment "1 9  Circumstances in which alternative procedure standard or other requirement is taken to meet requirements of Australian Meat Standard - Abrievated Graph Key: I13"@en-AU ;
    skos:definition "1 9  Circumstances in which alternative procedure standard or other requirement is taken to meet requirements of Australian Meat Standard"@en-AU ;
    skos:narrower F2021L00308:1 ;
    skos:prefLabel "Item I13"@en-AU ;
    dcat:accessURL <https://www.legislation.gov.au/F2021L00308/2023-08-04/2023-08-04/text/original/epub/OEBPS/document_1/document_1.html#_Toc143604722> ;
    dcat:landingPage "https://www.legislation.gov.au/F2021L00308/2023-08-04/2023-08-04/text/original/epub/OEBPS/document_1/document_1.html#_Toc143604722"^^xsd:anyURI ;
    dcat:theme legcons:Item .

F2021L00308:130 a legcons:Item,
        owl:Class,
        dcat:Resource ;
    rdfs:label "Item - I130 5 36  Export market eligibility"@en-AU ;
    dct:isPartOf F2021L00308:84 ;
    dct:isReferencedBy F2021L00308: ;
    rdfs:comment "5 36  Export market eligibility - Abrievated Graph Key: I130"@en-AU ;
    skos:definition "5 36  Export market eligibility"@en-AU ;
    skos:narrower F2021L00308:84 ;
    skos:prefLabel "Item I130"@en-AU ;
    dcat:accessURL <https://www.legislation.gov.au/F2021L00308/2023-08-04/2023-08-04/text/original/epub/OEBPS/document_1/document_1.html#_Toc143604839> ;
    dcat:landingPage "https://www.legislation.gov.au/F2021L00308/2023-08-04/2023-08-04/text/original/epub/OEBPS/document_1/document_1.html#_Toc143604839"^^xsd:anyURI ;
    dcat:theme legcons:Item .

F2021L00308:131 a legcons:Item,
        owl:Class,
        dcat:Resource ;
    rdfs:label "Item - I131 5 37  Action if prescribed rabbit meat ratite meat rabbit meat products or ratite meat products are unwholesome or integrity etc cannot be ensured"@en-AU ;
    dct:isPartOf F2021L00308:84 ;
    dct:isReferencedBy F2021L00308: ;
    rdfs:comment "5 37  Action if prescribed rabbit meat ratite meat rabbit meat products or ratite meat products are unwholesome or integrity etc cannot be ensured - Abrievated Graph Key: I131"@en-AU ;
    skos:definition "5 37  Action if prescribed rabbit meat ratite meat rabbit meat products or ratite meat products are unwholesome or integrity etc cannot be ensured"@en-AU ;
    skos:narrower F2021L00308:84 ;
    skos:prefLabel "Item I131"@en-AU ;
    dcat:accessURL <https://www.legislation.gov.au/F2021L00308/2023-08-04/2023-08-04/text/original/epub/OEBPS/document_1/document_1.html#_Toc143604840> ;
    dcat:landingPage "https://www.legislation.gov.au/F2021L00308/2023-08-04/2023-08-04/text/original/epub/OEBPS/document_1/document_1.html#_Toc143604840"^^xsd:anyURI ;
    dcat:theme legcons:Item .

F2021L00308:132 a legcons:Division,
        owl:Class,
        dcat:Resource ;
    rdfs:label "Division - D132 Division 8 Transfers"@en-AU ;
    dct:isPartOf F2021L00308:84 ;
    dct:isReferencedBy F2021L00308: ;
    rdfs:comment "Division 8 Transfers - Abrievated Graph Key: D132"@en-AU ;
    skos:definition "Division 8 Transfers"@en-AU ;
    skos:narrower F2021L00308:84 ;
    skos:prefLabel "Division D132"@en-AU ;
    dcat:accessURL <https://www.legislation.gov.au/F2021L00308/2023-08-04/2023-08-04/text/original/epub/OEBPS/document_1/document_1.html#_Toc143604841> ;
    dcat:landingPage "https://www.legislation.gov.au/F2021L00308/2023-08-04/2023-08-04/text/original/epub/OEBPS/document_1/document_1.html#_Toc143604841"^^xsd:anyURI ;
    dcat:theme legcons:Division .

F2021L00308:133 a legcons:Item,
        owl:Class,
        dcat:Resource ;
    rdfs:label "Item - I133 5 38  Information and declarations relating to transferred prescribed rabbit meat ratite meat rabbit meat products or ratite meat products"@en-AU ;
    dct:isPartOf F2021L00308:84 ;
    dct:isReferencedBy F2021L00308: ;
    rdfs:comment "5 38  Information and declarations relating to transferred prescribed rabbit meat ratite meat rabbit meat products or ratite meat products - Abrievated Graph Key: I133"@en-AU ;
    skos:definition "5 38  Information and declarations relating to transferred prescribed rabbit meat ratite meat rabbit meat products or ratite meat products"@en-AU ;
    skos:narrower F2021L00308:84 ;
    skos:prefLabel "Item I133"@en-AU ;
    dcat:accessURL <https://www.legislation.gov.au/F2021L00308/2023-08-04/2023-08-04/text/original/epub/OEBPS/document_1/document_1.html#_Toc143604842> ;
    dcat:landingPage "https://www.legislation.gov.au/F2021L00308/2023-08-04/2023-08-04/text/original/epub/OEBPS/document_1/document_1.html#_Toc143604842"^^xsd:anyURI ;
    dcat:theme legcons:Item .

F2021L00308:134 a legcons:Item,
        owl:Class,
        dcat:Resource ;
    rdfs:label "Item - I134 5 39  Information and declarations not received or inaccurate or incomplete"@en-AU ;
    dct:isPartOf F2021L00308:84 ;
    dct:isReferencedBy F2021L00308: ;
    rdfs:comment "5 39  Information and declarations not received or inaccurate or incomplete - Abrievated Graph Key: I134"@en-AU ;
    skos:definition "5 39  Information and declarations not received or inaccurate or incomplete"@en-AU ;
    skos:narrower F2021L00308:84 ;
    skos:prefLabel "Item I134"@en-AU ;
    dcat:accessURL <https://www.legislation.gov.au/F2021L00308/2023-08-04/2023-08-04/text/original/epub/OEBPS/document_1/document_1.html#_Toc143604843> ;
    dcat:landingPage "https://www.legislation.gov.au/F2021L00308/2023-08-04/2023-08-04/text/original/epub/OEBPS/document_1/document_1.html#_Toc143604843"^^xsd:anyURI ;
    dcat:theme legcons:Item .

F2021L00308:135 a legcons:Division,
        owl:Class,
        dcat:Resource ;
    rdfs:label "Division - D135 Division 9 Meat inspection services"@en-AU ;
    dct:isPartOf F2021L00308:84 ;
    dct:isReferencedBy F2021L00308: ;
    rdfs:comment "Division 9 Meat inspection services - Abrievated Graph Key: D135"@en-AU ;
    skos:definition "Division 9 Meat inspection services"@en-AU ;
    skos:narrower F2021L00308:84 ;
    skos:prefLabel "Division D135"@en-AU ;
    dcat:accessURL <https://www.legislation.gov.au/F2021L00308/2023-08-04/2023-08-04/text/original/epub/OEBPS/document_1/document_1.html#_Toc143604844> ;
    dcat:landingPage "https://www.legislation.gov.au/F2021L00308/2023-08-04/2023-08-04/text/original/epub/OEBPS/document_1/document_1.html#_Toc143604844"^^xsd:anyURI ;
    dcat:theme legcons:Division .

F2021L00308:136 a legcons:Item,
        owl:Class,
        dcat:Resource ;
    rdfs:label "Item - I136 5 40  Authorised officer must be present while certain export operations are carried out"@en-AU ;
    dct:isPartOf F2021L00308:84 ;
    dct:isReferencedBy F2021L00308: ;
    rdfs:comment "5 40  Authorised officer must be present while certain export operations are carried out - Abrievated Graph Key: I136"@en-AU ;
    skos:definition "5 40  Authorised officer must be present while certain export operations are carried out"@en-AU ;
    skos:narrower F2021L00308:84 ;
    skos:prefLabel "Item I136"@en-AU ;
    dcat:accessURL <https://www.legislation.gov.au/F2021L00308/2023-08-04/2023-08-04/text/original/epub/OEBPS/document_1/document_1.html#_Toc143604845> ;
    dcat:landingPage "https://www.legislation.gov.au/F2021L00308/2023-08-04/2023-08-04/text/original/epub/OEBPS/document_1/document_1.html#_Toc143604845"^^xsd:anyURI ;
    dcat:theme legcons:Item .

F2021L00308:137 a legcons:Division,
        owl:Class,
        dcat:Resource ;
    rdfs:label "Division - D137 Division 10 Management practices"@en-AU ;
    dct:isPartOf F2021L00308:84 ;
    dct:isReferencedBy F2021L00308: ;
    rdfs:comment "Division 10 Management practices - Abrievated Graph Key: D137"@en-AU ;
    skos:definition "Division 10 Management practices"@en-AU ;
    skos:narrower F2021L00308:84 ;
    skos:prefLabel "Division D137"@en-AU ;
    dcat:accessURL <https://www.legislation.gov.au/F2021L00308/2023-08-04/2023-08-04/text/original/epub/OEBPS/document_1/document_1.html#_Toc143604846> ;
    dcat:landingPage "https://www.legislation.gov.au/F2021L00308/2023-08-04/2023-08-04/text/original/epub/OEBPS/document_1/document_1.html#_Toc143604846"^^xsd:anyURI ;
    dcat:theme legcons:Division .

F2021L00308:138 a legcons:Item,
        owl:Class,
        dcat:Resource ;
    rdfs:label "Item - I138 5 41  Management practices organisational structure resources and personnel"@en-AU ;
    dct:isPartOf F2021L00308:84 ;
    dct:isReferencedBy F2021L00308: ;
    rdfs:comment "5 41  Management practices organisational structure resources and personnel - Abrievated Graph Key: I138"@en-AU ;
    skos:definition "5 41  Management practices organisational structure resources and personnel"@en-AU ;
    skos:narrower F2021L00308:84 ;
    skos:prefLabel "Item I138"@en-AU ;
    dcat:accessURL <https://www.legislation.gov.au/F2021L00308/2023-08-04/2023-08-04/text/original/epub/OEBPS/document_1/document_1.html#_Toc143604847> ;
    dcat:landingPage "https://www.legislation.gov.au/F2021L00308/2023-08-04/2023-08-04/text/original/epub/OEBPS/document_1/document_1.html#_Toc143604847"^^xsd:anyURI ;
    dcat:theme legcons:Item .

F2021L00308:139 a legcons:Item,
        owl:Class,
        dcat:Resource ;
    rdfs:label "Item - I139 5 42  Verification of compliance with the Act and other matters"@en-AU ;
    dct:isPartOf F2021L00308:84 ;
    dct:isReferencedBy F2021L00308: ;
    rdfs:comment "5 42  Verification of compliance with the Act and other matters - Abrievated Graph Key: I139"@en-AU ;
    skos:definition "5 42  Verification of compliance with the Act and other matters"@en-AU ;
    skos:narrower F2021L00308:84 ;
    skos:prefLabel "Item I139"@en-AU ;
    dcat:accessURL <https://www.legislation.gov.au/F2021L00308/2023-08-04/2023-08-04/text/original/epub/OEBPS/document_1/document_1.html#_Toc143604848> ;
    dcat:landingPage "https://www.legislation.gov.au/F2021L00308/2023-08-04/2023-08-04/text/original/epub/OEBPS/document_1/document_1.html#_Toc143604848"^^xsd:anyURI ;
    dcat:theme legcons:Item .

F2021L00308:140 a legcons:Item,
        owl:Class,
        dcat:Resource ;
    rdfs:label "Item - I140 5 43  Action must be taken to address non compliance"@en-AU ;
    dct:isPartOf F2021L00308:84 ;
    dct:isReferencedBy F2021L00308: ;
    rdfs:comment "5 43  Action must be taken to address non compliance - Abrievated Graph Key: I140"@en-AU ;
    skos:definition "5 43  Action must be taken to address non compliance"@en-AU ;
    skos:narrower F2021L00308:84 ;
    skos:prefLabel "Item I140"@en-AU ;
    dcat:accessURL <https://www.legislation.gov.au/F2021L00308/2023-08-04/2023-08-04/text/original/epub/OEBPS/document_1/document_1.html#_Toc143604849> ;
    dcat:landingPage "https://www.legislation.gov.au/F2021L00308/2023-08-04/2023-08-04/text/original/epub/OEBPS/document_1/document_1.html#_Toc143604849"^^xsd:anyURI ;
    dcat:theme legcons:Item .

F2021L00308:141 a legcons:Item,
        owl:Class,
        dcat:Resource ;
    rdfs:label "Item - I141 5 44  Internal audit and management review"@en-AU ;
    dct:isPartOf F2021L00308:84 ;
    dct:isReferencedBy F2021L00308: ;
    rdfs:comment "5 44  Internal audit and management review - Abrievated Graph Key: I141"@en-AU ;
    skos:definition "5 44  Internal audit and management review"@en-AU ;
    skos:narrower F2021L00308:84 ;
    skos:prefLabel "Item I141"@en-AU ;
    dcat:accessURL <https://www.legislation.gov.au/F2021L00308/2023-08-04/2023-08-04/text/original/epub/OEBPS/document_1/document_1.html#_Toc143604850> ;
    dcat:landingPage "https://www.legislation.gov.au/F2021L00308/2023-08-04/2023-08-04/text/original/epub/OEBPS/document_1/document_1.html#_Toc143604850"^^xsd:anyURI ;
    dcat:theme legcons:Item .

F2021L00308:142 a legcons:Part,
        owl:Class,
        dcat:Resource ;
    rdfs:label "Part - P142 Part 3 Renewal of approved arrangement"@en-AU ;
    dct:isPartOf F2021L00308:80 ;
    dct:isReferencedBy F2021L00308: ;
    rdfs:comment "Part 3 Renewal of approved arrangement - Abrievated Graph Key: P142"@en-AU ;
    skos:definition "Part 3 Renewal of approved arrangement"@en-AU ;
    skos:narrower F2021L00308:80 ;
    skos:prefLabel "Part P142"@en-AU ;
    dcat:accessURL <https://www.legislation.gov.au/F2021L00308/2023-08-04/2023-08-04/text/original/epub/OEBPS/document_1/document_1.html#_Toc143604851> ;
    dcat:landingPage "https://www.legislation.gov.au/F2021L00308/2023-08-04/2023-08-04/text/original/epub/OEBPS/document_1/document_1.html#_Toc143604851"^^xsd:anyURI ;
    dcat:theme legcons:Part .

F2021L00308:143 a legcons:Item,
        owl:Class,
        dcat:Resource ;
    rdfs:label "Item - I143 5 45  Period within which application to renew approved arrangement must be made"@en-AU ;
    dct:isPartOf F2021L00308:80 ;
    dct:isReferencedBy F2021L00308: ;
    rdfs:comment "5 45  Period within which application to renew approved arrangement must be made - Abrievated Graph Key: I143"@en-AU ;
    skos:definition "5 45  Period within which application to renew approved arrangement must be made"@en-AU ;
    skos:narrower F2021L00308:80 ;
    skos:prefLabel "Item I143"@en-AU ;
    dcat:accessURL <https://www.legislation.gov.au/F2021L00308/2023-08-04/2023-08-04/text/original/epub/OEBPS/document_1/document_1.html#_Toc143604852> ;
    dcat:landingPage "https://www.legislation.gov.au/F2021L00308/2023-08-04/2023-08-04/text/original/epub/OEBPS/document_1/document_1.html#_Toc143604852"^^xsd:anyURI ;
    dcat:theme legcons:Item .

F2021L00308:144 a legcons:Part,
        owl:Class,
        dcat:Resource ;
    rdfs:label "Part - P144 Part 4 Variation of approved arrangement"@en-AU ;
    dct:isPartOf F2021L00308:80 ;
    dct:isReferencedBy F2021L00308: ;
    rdfs:comment "Part 4 Variation of approved arrangement - Abrievated Graph Key: P144"@en-AU ;
    skos:definition "Part 4 Variation of approved arrangement"@en-AU ;
    skos:narrower F2021L00308:80 ;
    skos:prefLabel "Part P144"@en-AU ;
    dcat:accessURL <https://www.legislation.gov.au/F2021L00308/2023-08-04/2023-08-04/text/original/epub/OEBPS/document_1/document_1.html#_Toc143604853> ;
    dcat:landingPage "https://www.legislation.gov.au/F2021L00308/2023-08-04/2023-08-04/text/original/epub/OEBPS/document_1/document_1.html#_Toc143604853"^^xsd:anyURI ;
    dcat:theme legcons:Part .

F2021L00308:146 a legcons:Item,
        owl:Class,
        dcat:Resource ;
    rdfs:label "Item - I146 5 46  Requirements that must be met for variation to be approved or conditions varied"@en-AU ;
    dct:isPartOf F2021L00308:145 ;
    dct:isReferencedBy F2021L00308: ;
    rdfs:comment "5 46  Requirements that must be met for variation to be approved or conditions varied - Abrievated Graph Key: I146"@en-AU ;
    skos:definition "5 46  Requirements that must be met for variation to be approved or conditions varied"@en-AU ;
    skos:narrower F2021L00308:145 ;
    skos:prefLabel "Item I146"@en-AU ;
    dcat:accessURL <https://www.legislation.gov.au/F2021L00308/2023-08-04/2023-08-04/text/original/epub/OEBPS/document_1/document_1.html#_Toc143604855> ;
    dcat:landingPage "https://www.legislation.gov.au/F2021L00308/2023-08-04/2023-08-04/text/original/epub/OEBPS/document_1/document_1.html#_Toc143604855"^^xsd:anyURI ;
    dcat:theme legcons:Item .

F2021L00308:147 a legcons:Item,
        owl:Class,
        dcat:Resource ;
    rdfs:label "Item - I147 5 47  Significant variations"@en-AU ;
    dct:isPartOf F2021L00308:145 ;
    dct:isReferencedBy F2021L00308: ;
    rdfs:comment "5 47  Significant variations - Abrievated Graph Key: I147"@en-AU ;
    skos:definition "5 47  Significant variations"@en-AU ;
    skos:narrower F2021L00308:145 ;
    skos:prefLabel "Item I147"@en-AU ;
    dcat:accessURL <https://www.legislation.gov.au/F2021L00308/2023-08-04/2023-08-04/text/original/epub/OEBPS/document_1/document_1.html#_Toc143604856> ;
    dcat:landingPage "https://www.legislation.gov.au/F2021L00308/2023-08-04/2023-08-04/text/original/epub/OEBPS/document_1/document_1.html#_Toc143604856"^^xsd:anyURI ;
    dcat:theme legcons:Item .

F2021L00308:149 a legcons:Item,
        owl:Class,
        dcat:Resource ;
    rdfs:label "Item - I149 5 48  Other reasons for requiring holder to vary approved arrangement"@en-AU ;
    dct:isPartOf F2021L00308:148 ;
    dct:isReferencedBy F2021L00308: ;
    rdfs:comment "5 48  Other reasons for requiring holder to vary approved arrangement - Abrievated Graph Key: I149"@en-AU ;
    skos:definition "5 48  Other reasons for requiring holder to vary approved arrangement"@en-AU ;
    skos:narrower F2021L00308:148 ;
    skos:prefLabel "Item I149"@en-AU ;
    dcat:accessURL <https://www.legislation.gov.au/F2021L00308/2023-08-04/2023-08-04/text/original/epub/OEBPS/document_1/document_1.html#_Toc143604858> ;
    dcat:landingPage "https://www.legislation.gov.au/F2021L00308/2023-08-04/2023-08-04/text/original/epub/OEBPS/document_1/document_1.html#_Toc143604858"^^xsd:anyURI ;
    dcat:theme legcons:Item .

F2021L00308:150 a legcons:Part,
        owl:Class,
        dcat:Resource ;
    rdfs:label "Part - P150 Part 5 Matters relating to applications"@en-AU ;
    dct:isPartOf F2021L00308:80 ;
    dct:isReferencedBy F2021L00308: ;
    rdfs:comment "Part 5 Matters relating to applications - Abrievated Graph Key: P150"@en-AU ;
    skos:definition "Part 5 Matters relating to applications"@en-AU ;
    skos:narrower F2021L00308:80 ;
    skos:prefLabel "Part P150"@en-AU ;
    dcat:accessURL <https://www.legislation.gov.au/F2021L00308/2023-08-04/2023-08-04/text/original/epub/OEBPS/document_1/document_1.html#_Toc143604859> ;
    dcat:landingPage "https://www.legislation.gov.au/F2021L00308/2023-08-04/2023-08-04/text/original/epub/OEBPS/document_1/document_1.html#_Toc143604859"^^xsd:anyURI ;
    dcat:theme legcons:Part .

F2021L00308:151 a legcons:Item,
        owl:Class,
        dcat:Resource ;
    rdfs:label "Item - I151 5 49  Application of this Part"@en-AU ;
    dct:isPartOf F2021L00308:80 ;
    dct:isReferencedBy F2021L00308: ;
    rdfs:comment "5 49  Application of this Part - Abrievated Graph Key: I151"@en-AU ;
    skos:definition "5 49  Application of this Part"@en-AU ;
    skos:narrower F2021L00308:80 ;
    skos:prefLabel "Item I151"@en-AU ;
    dcat:accessURL <https://www.legislation.gov.au/F2021L00308/2023-08-04/2023-08-04/text/original/epub/OEBPS/document_1/document_1.html#_Toc143604860> ;
    dcat:landingPage "https://www.legislation.gov.au/F2021L00308/2023-08-04/2023-08-04/text/original/epub/OEBPS/document_1/document_1.html#_Toc143604860"^^xsd:anyURI ;
    dcat:theme legcons:Item .

F2021L00308:152 a legcons:Item,
        owl:Class,
        dcat:Resource ;
    rdfs:label "Item - I152 5 50  Initial consideration period"@en-AU ;
    dct:isPartOf F2021L00308:80 ;
    dct:isReferencedBy F2021L00308: ;
    rdfs:comment "5 50  Initial consideration period - Abrievated Graph Key: I152"@en-AU ;
    skos:definition "5 50  Initial consideration period"@en-AU ;
    skos:narrower F2021L00308:80 ;
    skos:prefLabel "Item I152"@en-AU ;
    dcat:accessURL <https://www.legislation.gov.au/F2021L00308/2023-08-04/2023-08-04/text/original/epub/OEBPS/document_1/document_1.html#_Toc143604861> ;
    dcat:landingPage "https://www.legislation.gov.au/F2021L00308/2023-08-04/2023-08-04/text/original/epub/OEBPS/document_1/document_1.html#_Toc143604861"^^xsd:anyURI ;
    dcat:theme legcons:Item .

F2021L00308:153 a legcons:Item,
        owl:Class,
        dcat:Resource ;
    rdfs:label "Item - I153 5 51  Period within which request relating to application must be complied with"@en-AU ;
    dct:isPartOf F2021L00308:80 ;
    dct:isReferencedBy F2021L00308: ;
    rdfs:comment "5 51  Period within which request relating to application must be complied with - Abrievated Graph Key: I153"@en-AU ;
    skos:definition "5 51  Period within which request relating to application must be complied with"@en-AU ;
    skos:narrower F2021L00308:80 ;
    skos:prefLabel "Item I153"@en-AU ;
    dcat:accessURL <https://www.legislation.gov.au/F2021L00308/2023-08-04/2023-08-04/text/original/epub/OEBPS/document_1/document_1.html#_Toc143604862> ;
    dcat:landingPage "https://www.legislation.gov.au/F2021L00308/2023-08-04/2023-08-04/text/original/epub/OEBPS/document_1/document_1.html#_Toc143604862"^^xsd:anyURI ;
    dcat:theme legcons:Item .

F2021L00308:156 a legcons:Item,
        owl:Class,
        dcat:Resource ;
    rdfs:label "Item - I156 7 1  Period of effect of export permit"@en-AU ;
    dct:isPartOf F2021L00308:155 ;
    dct:isReferencedBy F2021L00308: ;
    rdfs:comment "7 1  Period of effect of export permit - Abrievated Graph Key: I156"@en-AU ;
    skos:definition "7 1  Period of effect of export permit"@en-AU ;
    skos:narrower F2021L00308:155 ;
    skos:prefLabel "Item I156"@en-AU ;
    dcat:accessURL <https://www.legislation.gov.au/F2021L00308/2023-08-04/2023-08-04/text/original/epub/OEBPS/document_1/document_1.html#_Toc143604865> ;
    dcat:landingPage "https://www.legislation.gov.au/F2021L00308/2023-08-04/2023-08-04/text/original/epub/OEBPS/document_1/document_1.html#_Toc143604865"^^xsd:anyURI ;
    dcat:theme legcons:Item .

F2021L00308:158 a legcons:Item,
        owl:Class,
        dcat:Resource ;
    rdfs:label "Item - I158 7 2  Period of effect of varied export permit"@en-AU ;
    dct:isPartOf F2021L00308:157 ;
    dct:isReferencedBy F2021L00308: ;
    rdfs:comment "7 2  Period of effect of varied export permit - Abrievated Graph Key: I158"@en-AU ;
    skos:definition "7 2  Period of effect of varied export permit"@en-AU ;
    skos:narrower F2021L00308:157 ;
    skos:prefLabel "Item I158"@en-AU ;
    dcat:accessURL <https://www.legislation.gov.au/F2021L00308/2023-08-04/2023-08-04/text/original/epub/OEBPS/document_1/document_1.html#_Toc143604867> ;
    dcat:landingPage "https://www.legislation.gov.au/F2021L00308/2023-08-04/2023-08-04/text/original/epub/OEBPS/document_1/document_1.html#_Toc143604867"^^xsd:anyURI ;
    dcat:theme legcons:Item .

F2021L00308:159 a legcons:Item,
        owl:Class,
        dcat:Resource ;
    rdfs:label "Item - I159 7 3  Circumstances in which export permit may be suspended"@en-AU ;
    dct:isPartOf F2021L00308:157 ;
    dct:isReferencedBy F2021L00308: ;
    rdfs:comment "7 3  Circumstances in which export permit may be suspended - Abrievated Graph Key: I159"@en-AU ;
    skos:definition "7 3  Circumstances in which export permit may be suspended"@en-AU ;
    skos:narrower F2021L00308:157 ;
    skos:prefLabel "Item I159"@en-AU ;
    dcat:accessURL <https://www.legislation.gov.au/F2021L00308/2023-08-04/2023-08-04/text/original/epub/OEBPS/document_1/document_1.html#_Toc143604868> ;
    dcat:landingPage "https://www.legislation.gov.au/F2021L00308/2023-08-04/2023-08-04/text/original/epub/OEBPS/document_1/document_1.html#_Toc143604868"^^xsd:anyURI ;
    dcat:theme legcons:Item .

F2021L00308:160 a legcons:Item,
        owl:Class,
        dcat:Resource ;
    rdfs:label "Item - I160 7 4  Other circumstances in which export permit may be revoked"@en-AU ;
    dct:isPartOf F2021L00308:157 ;
    dct:isReferencedBy F2021L00308: ;
    rdfs:comment "7 4  Other circumstances in which export permit may be revoked - Abrievated Graph Key: I160"@en-AU ;
    skos:definition "7 4  Other circumstances in which export permit may be revoked"@en-AU ;
    skos:narrower F2021L00308:157 ;
    skos:prefLabel "Item I160"@en-AU ;
    dcat:accessURL <https://www.legislation.gov.au/F2021L00308/2023-08-04/2023-08-04/text/original/epub/OEBPS/document_1/document_1.html#_Toc143604869> ;
    dcat:landingPage "https://www.legislation.gov.au/F2021L00308/2023-08-04/2023-08-04/text/original/epub/OEBPS/document_1/document_1.html#_Toc143604869"^^xsd:anyURI ;
    dcat:theme legcons:Item .

F2021L00308:162 a legcons:Item,
        owl:Class,
        dcat:Resource ;
    rdfs:label "Item - I162 7 5  Changes that require additional or corrected information to be given to the Secretary"@en-AU ;
    dct:isPartOf F2021L00308:161 ;
    dct:isReferencedBy F2021L00308: ;
    rdfs:comment "7 5  Changes that require additional or corrected information to be given to the Secretary - Abrievated Graph Key: I162"@en-AU ;
    skos:definition "7 5  Changes that require additional or corrected information to be given to the Secretary"@en-AU ;
    skos:narrower F2021L00308:161 ;
    skos:prefLabel "Item I162"@en-AU ;
    dcat:accessURL <https://www.legislation.gov.au/F2021L00308/2023-08-04/2023-08-04/text/original/epub/OEBPS/document_1/document_1.html#_Toc143604871> ;
    dcat:landingPage "https://www.legislation.gov.au/F2021L00308/2023-08-04/2023-08-04/text/original/epub/OEBPS/document_1/document_1.html#_Toc143604871"^^xsd:anyURI ;
    dcat:theme legcons:Item .

F2021L00308:163 a legcons:Item,
        owl:Class,
        dcat:Resource ;
    rdfs:label "Item - I163 7 6  Return of export permit"@en-AU ;
    dct:isPartOf F2021L00308:161 ;
    dct:isReferencedBy F2021L00308: ;
    rdfs:comment "7 6  Return of export permit - Abrievated Graph Key: I163"@en-AU ;
    skos:definition "7 6  Return of export permit"@en-AU ;
    skos:narrower F2021L00308:161 ;
    skos:prefLabel "Item I163"@en-AU ;
    dcat:accessURL <https://www.legislation.gov.au/F2021L00308/2023-08-04/2023-08-04/text/original/epub/OEBPS/document_1/document_1.html#_Toc143604872> ;
    dcat:landingPage "https://www.legislation.gov.au/F2021L00308/2023-08-04/2023-08-04/text/original/epub/OEBPS/document_1/document_1.html#_Toc143604872"^^xsd:anyURI ;
    dcat:theme legcons:Item .

F2021L00308:164 a legcons:Item,
        owl:Class,
        dcat:Resource ;
    rdfs:label "Item - I164 7 7  Notification that prescribed rabbit meat ratite meat rabbit meat products or ratite meat products are not to be exported"@en-AU ;
    dct:isPartOf F2021L00308:161 ;
    dct:isReferencedBy F2021L00308: ;
    rdfs:comment "7 7  Notification that prescribed rabbit meat ratite meat rabbit meat products or ratite meat products are not to be exported - Abrievated Graph Key: I164"@en-AU ;
    skos:definition "7 7  Notification that prescribed rabbit meat ratite meat rabbit meat products or ratite meat products are not to be exported"@en-AU ;
    skos:narrower F2021L00308:161 ;
    skos:prefLabel "Item I164"@en-AU ;
    dcat:accessURL <https://www.legislation.gov.au/F2021L00308/2023-08-04/2023-08-04/text/original/epub/OEBPS/document_1/document_1.html#_Toc143604873> ;
    dcat:landingPage "https://www.legislation.gov.au/F2021L00308/2023-08-04/2023-08-04/text/original/epub/OEBPS/document_1/document_1.html#_Toc143604873"^^xsd:anyURI ;
    dcat:theme legcons:Item .

F2021L00308:165 a legcons:Item,
        owl:Class,
        dcat:Resource ;
    rdfs:label "Item - I165 7 8  Application for export permit must include declaration"@en-AU ;
    dct:isPartOf F2021L00308:161 ;
    dct:isReferencedBy F2021L00308: ;
    rdfs:comment "7 8  Application for export permit must include declaration - Abrievated Graph Key: I165"@en-AU ;
    skos:definition "7 8  Application for export permit must include declaration"@en-AU ;
    skos:narrower F2021L00308:161 ;
    skos:prefLabel "Item I165"@en-AU ;
    dcat:accessURL <https://www.legislation.gov.au/F2021L00308/2023-08-04/2023-08-04/text/original/epub/OEBPS/document_1/document_1.html#_Toc143604874> ;
    dcat:landingPage "https://www.legislation.gov.au/F2021L00308/2023-08-04/2023-08-04/text/original/epub/OEBPS/document_1/document_1.html#_Toc143604874"^^xsd:anyURI ;
    dcat:theme legcons:Item .

F2021L00308:168 a legcons:Item,
        owl:Class,
        dcat:Resource ;
    rdfs:label "Item - I168 8 1  Information to be included in notice of intention to export"@en-AU ;
    dct:isPartOf F2021L00308:167 ;
    dct:isReferencedBy F2021L00308: ;
    rdfs:comment "8 1  Information to be included in notice of intention to export - Abrievated Graph Key: I168"@en-AU ;
    skos:definition "8 1  Information to be included in notice of intention to export"@en-AU ;
    skos:narrower F2021L00308:167 ;
    skos:prefLabel "Item I168"@en-AU ;
    dcat:accessURL <https://www.legislation.gov.au/F2021L00308/2023-08-04/2023-08-04/text/original/epub/OEBPS/document_1/document_1.html#_Toc143604877> ;
    dcat:landingPage "https://www.legislation.gov.au/F2021L00308/2023-08-04/2023-08-04/text/original/epub/OEBPS/document_1/document_1.html#_Toc143604877"^^xsd:anyURI ;
    dcat:theme legcons:Item .

F2021L00308:169 a legcons:Item,
        owl:Class,
        dcat:Resource ;
    rdfs:label "Item - I169 8 2  Person who must give notice of intention to export"@en-AU ;
    dct:isPartOf F2021L00308:167 ;
    dct:isReferencedBy F2021L00308: ;
    rdfs:comment "8 2  Person who must give notice of intention to export - Abrievated Graph Key: I169"@en-AU ;
    skos:definition "8 2  Person who must give notice of intention to export"@en-AU ;
    skos:narrower F2021L00308:167 ;
    skos:prefLabel "Item I169"@en-AU ;
    dcat:accessURL <https://www.legislation.gov.au/F2021L00308/2023-08-04/2023-08-04/text/original/epub/OEBPS/document_1/document_1.html#_Toc143604878> ;
    dcat:landingPage "https://www.legislation.gov.au/F2021L00308/2023-08-04/2023-08-04/text/original/epub/OEBPS/document_1/document_1.html#_Toc143604878"^^xsd:anyURI ;
    dcat:theme legcons:Item .

F2021L00308:17 a legcons:Item,
        owl:Class,
        dcat:Resource ;
    rdfs:label "Item - I17 2 1  Rabbit meat ratite meat rabbit meat products and ratite meat products that are prescribed goods"@en-AU ;
    dct:isPartOf F2021L00308:16 ;
    dct:isReferencedBy F2021L00308: ;
    rdfs:comment "2 1  Rabbit meat ratite meat rabbit meat products and ratite meat products that are prescribed goods - Abrievated Graph Key: I17"@en-AU ;
    skos:definition "2 1  Rabbit meat ratite meat rabbit meat products and ratite meat products that are prescribed goods"@en-AU ;
    skos:narrower F2021L00308:16 ;
    skos:prefLabel "Item I17"@en-AU ;
    dcat:accessURL <https://www.legislation.gov.au/F2021L00308/2023-08-04/2023-08-04/text/original/epub/OEBPS/document_1/document_1.html#_Toc143604726> ;
    dcat:landingPage "https://www.legislation.gov.au/F2021L00308/2023-08-04/2023-08-04/text/original/epub/OEBPS/document_1/document_1.html#_Toc143604726"^^xsd:anyURI ;
    dcat:theme legcons:Item .

F2021L00308:170 a legcons:Item,
        owl:Class,
        dcat:Resource ;
    rdfs:label "Item - I170 8 3  Person to whom notice of intention to export must be given"@en-AU ;
    dct:isPartOf F2021L00308:167 ;
    dct:isReferencedBy F2021L00308: ;
    rdfs:comment "8 3  Person to whom notice of intention to export must be given - Abrievated Graph Key: I170"@en-AU ;
    skos:definition "8 3  Person to whom notice of intention to export must be given"@en-AU ;
    skos:narrower F2021L00308:167 ;
    skos:prefLabel "Item I170"@en-AU ;
    dcat:accessURL <https://www.legislation.gov.au/F2021L00308/2023-08-04/2023-08-04/text/original/epub/OEBPS/document_1/document_1.html#_Toc143604879> ;
    dcat:landingPage "https://www.legislation.gov.au/F2021L00308/2023-08-04/2023-08-04/text/original/epub/OEBPS/document_1/document_1.html#_Toc143604879"^^xsd:anyURI ;
    dcat:theme legcons:Item .

F2021L00308:171 a legcons:Item,
        owl:Class,
        dcat:Resource ;
    rdfs:label "Item - I171 8 4  When notice of intention to export must be given"@en-AU ;
    dct:isPartOf F2021L00308:167 ;
    dct:isReferencedBy F2021L00308: ;
    rdfs:comment "8 4  When notice of intention to export must be given - Abrievated Graph Key: I171"@en-AU ;
    skos:definition "8 4  When notice of intention to export must be given"@en-AU ;
    skos:narrower F2021L00308:167 ;
    skos:prefLabel "Item I171"@en-AU ;
    dcat:accessURL <https://www.legislation.gov.au/F2021L00308/2023-08-04/2023-08-04/text/original/epub/OEBPS/document_1/document_1.html#_Toc143604880> ;
    dcat:landingPage "https://www.legislation.gov.au/F2021L00308/2023-08-04/2023-08-04/text/original/epub/OEBPS/document_1/document_1.html#_Toc143604880"^^xsd:anyURI ;
    dcat:theme legcons:Item .

F2021L00308:173 a legcons:Item,
        owl:Class,
        dcat:Resource ;
    rdfs:label "Item - I173 8 5  Purpose of this Part"@en-AU ;
    dct:isPartOf F2021L00308:172 ;
    dct:isReferencedBy F2021L00308: ;
    rdfs:comment "8 5  Purpose of this Part - Abrievated Graph Key: I173"@en-AU ;
    skos:definition "8 5  Purpose of this Part"@en-AU ;
    skos:narrower F2021L00308:172 ;
    skos:prefLabel "Item I173"@en-AU ;
    dcat:accessURL <https://www.legislation.gov.au/F2021L00308/2023-08-04/2023-08-04/text/original/epub/OEBPS/document_1/document_1.html#_Toc143604882> ;
    dcat:landingPage "https://www.legislation.gov.au/F2021L00308/2023-08-04/2023-08-04/text/original/epub/OEBPS/document_1/document_1.html#_Toc143604882"^^xsd:anyURI ;
    dcat:theme legcons:Item .

F2021L00308:174 a legcons:Item,
        owl:Class,
        dcat:Resource ;
    rdfs:label "Item - I174 8 6  General requirements for trade descriptions"@en-AU ;
    dct:isPartOf F2021L00308:172 ;
    dct:isReferencedBy F2021L00308: ;
    rdfs:comment "8 6  General requirements for trade descriptions - Abrievated Graph Key: I174"@en-AU ;
    skos:definition "8 6  General requirements for trade descriptions"@en-AU ;
    skos:narrower F2021L00308:172 ;
    skos:prefLabel "Item I174"@en-AU ;
    dcat:accessURL <https://www.legislation.gov.au/F2021L00308/2023-08-04/2023-08-04/text/original/epub/OEBPS/document_1/document_1.html#_Toc143604883> ;
    dcat:landingPage "https://www.legislation.gov.au/F2021L00308/2023-08-04/2023-08-04/text/original/epub/OEBPS/document_1/document_1.html#_Toc143604883"^^xsd:anyURI ;
    dcat:theme legcons:Item .

F2021L00308:175 a legcons:Item,
        owl:Class,
        dcat:Resource ;
    rdfs:label "Item - I175 8 7  Trade descriptions in language other than English"@en-AU ;
    dct:isPartOf F2021L00308:172 ;
    dct:isReferencedBy F2021L00308: ;
    rdfs:comment "8 7  Trade descriptions in language other than English - Abrievated Graph Key: I175"@en-AU ;
    skos:definition "8 7  Trade descriptions in language other than English"@en-AU ;
    skos:narrower F2021L00308:172 ;
    skos:prefLabel "Item I175"@en-AU ;
    dcat:accessURL <https://www.legislation.gov.au/F2021L00308/2023-08-04/2023-08-04/text/original/epub/OEBPS/document_1/document_1.html#_Toc143604884> ;
    dcat:landingPage "https://www.legislation.gov.au/F2021L00308/2023-08-04/2023-08-04/text/original/epub/OEBPS/document_1/document_1.html#_Toc143604884"^^xsd:anyURI ;
    dcat:theme legcons:Item .

F2021L00308:178 a legcons:Item,
        owl:Class,
        dcat:Resource ;
    rdfs:label "Item - I178 8 8  Purpose of this Division"@en-AU ;
    dct:isPartOf F2021L00308:177 ;
    dct:isReferencedBy F2021L00308: ;
    rdfs:comment "8 8  Purpose of this Division - Abrievated Graph Key: I178"@en-AU ;
    skos:definition "8 8  Purpose of this Division"@en-AU ;
    skos:narrower F2021L00308:177 ;
    skos:prefLabel "Item I178"@en-AU ;
    dcat:accessURL <https://www.legislation.gov.au/F2021L00308/2023-08-04/2023-08-04/text/original/epub/OEBPS/document_1/document_1.html#_Toc143604887> ;
    dcat:landingPage "https://www.legislation.gov.au/F2021L00308/2023-08-04/2023-08-04/text/original/epub/OEBPS/document_1/document_1.html#_Toc143604887"^^xsd:anyURI ;
    dcat:theme legcons:Item .

F2021L00308:179 a legcons:Item,
        owl:Class,
        dcat:Resource ;
    rdfs:label "Item - I179 8 9  Tolerances for dimensions of official marks"@en-AU ;
    dct:isPartOf F2021L00308:177 ;
    dct:isReferencedBy F2021L00308: ;
    rdfs:comment "8 9  Tolerances for dimensions of official marks - Abrievated Graph Key: I179"@en-AU ;
    skos:definition "8 9  Tolerances for dimensions of official marks"@en-AU ;
    skos:narrower F2021L00308:177 ;
    skos:prefLabel "Item I179"@en-AU ;
    dcat:accessURL <https://www.legislation.gov.au/F2021L00308/2023-08-04/2023-08-04/text/original/epub/OEBPS/document_1/document_1.html#_Toc143604888> ;
    dcat:landingPage "https://www.legislation.gov.au/F2021L00308/2023-08-04/2023-08-04/text/original/epub/OEBPS/document_1/document_1.html#_Toc143604888"^^xsd:anyURI ;
    dcat:theme legcons:Item .

F2021L00308:18 a legcons:Item,
        owl:Class,
        dcat:Resource ;
    rdfs:label "Item - I18 2 2  Rabbit meat ratite meat rabbit meat products and ratite meat products that are taken not to be prescribed goods"@en-AU ;
    dct:isPartOf F2021L00308:16 ;
    dct:isReferencedBy F2021L00308: ;
    rdfs:comment "2 2  Rabbit meat ratite meat rabbit meat products and ratite meat products that are taken not to be prescribed goods - Abrievated Graph Key: I18"@en-AU ;
    skos:definition "2 2  Rabbit meat ratite meat rabbit meat products and ratite meat products that are taken not to be prescribed goods"@en-AU ;
    skos:narrower F2021L00308:16 ;
    skos:prefLabel "Item I18"@en-AU ;
    dcat:accessURL <https://www.legislation.gov.au/F2021L00308/2023-08-04/2023-08-04/text/original/epub/OEBPS/document_1/document_1.html#_Toc143604727> ;
    dcat:landingPage "https://www.legislation.gov.au/F2021L00308/2023-08-04/2023-08-04/text/original/epub/OEBPS/document_1/document_1.html#_Toc143604727"^^xsd:anyURI ;
    dcat:theme legcons:Item .

F2021L00308:180 a legcons:Item,
        owl:Class,
        dcat:Resource ;
    rdfs:label "Item - I180 8 10  Official markAustralia Inspected"@en-AU ;
    dct:isPartOf F2021L00308:177 ;
    dct:isReferencedBy F2021L00308: ;
    rdfs:comment "8 10  Official markAustralia Inspected - Abrievated Graph Key: I180"@en-AU ;
    skos:definition "8 10  Official markAustralia Inspected"@en-AU ;
    skos:narrower F2021L00308:177 ;
    skos:prefLabel "Item I180"@en-AU ;
    dcat:accessURL <https://www.legislation.gov.au/F2021L00308/2023-08-04/2023-08-04/text/original/epub/OEBPS/document_1/document_1.html#_Toc143604889> ;
    dcat:landingPage "https://www.legislation.gov.au/F2021L00308/2023-08-04/2023-08-04/text/original/epub/OEBPS/document_1/document_1.html#_Toc143604889"^^xsd:anyURI ;
    dcat:theme legcons:Item .

F2021L00308:181 a legcons:Item,
        owl:Class,
        dcat:Resource ;
    rdfs:label "Item - I181 8 11  Official markforeign country identification"@en-AU ;
    dct:isPartOf F2021L00308:177 ;
    dct:isReferencedBy F2021L00308: ;
    rdfs:comment "8 11  Official markforeign country identification - Abrievated Graph Key: I181"@en-AU ;
    skos:definition "8 11  Official markforeign country identification"@en-AU ;
    skos:narrower F2021L00308:177 ;
    skos:prefLabel "Item I181"@en-AU ;
    dcat:accessURL <https://www.legislation.gov.au/F2021L00308/2023-08-04/2023-08-04/text/original/epub/OEBPS/document_1/document_1.html#_Toc143604890> ;
    dcat:landingPage "https://www.legislation.gov.au/F2021L00308/2023-08-04/2023-08-04/text/original/epub/OEBPS/document_1/document_1.html#_Toc143604890"^^xsd:anyURI ;
    dcat:theme legcons:Item .

F2021L00308:182 a legcons:Item,
        owl:Class,
        dcat:Resource ;
    rdfs:label "Item - I182 8 12  Official marktamper indicative metal strap seal"@en-AU ;
    dct:isPartOf F2021L00308:177 ;
    dct:isReferencedBy F2021L00308: ;
    rdfs:comment "8 12  Official marktamper indicative metal strap seal - Abrievated Graph Key: I182"@en-AU ;
    skos:definition "8 12  Official marktamper indicative metal strap seal"@en-AU ;
    skos:narrower F2021L00308:177 ;
    skos:prefLabel "Item I182"@en-AU ;
    dcat:accessURL <https://www.legislation.gov.au/F2021L00308/2023-08-04/2023-08-04/text/original/epub/OEBPS/document_1/document_1.html#_Toc143604891> ;
    dcat:landingPage "https://www.legislation.gov.au/F2021L00308/2023-08-04/2023-08-04/text/original/epub/OEBPS/document_1/document_1.html#_Toc143604891"^^xsd:anyURI ;
    dcat:theme legcons:Item .

F2021L00308:183 a legcons:Item,
        owl:Class,
        dcat:Resource ;
    rdfs:label "Item - I183 8 13  Official markbolt seal"@en-AU ;
    dct:isPartOf F2021L00308:177 ;
    dct:isReferencedBy F2021L00308: ;
    rdfs:comment "8 13  Official markbolt seal - Abrievated Graph Key: I183"@en-AU ;
    skos:definition "8 13  Official markbolt seal"@en-AU ;
    skos:narrower F2021L00308:177 ;
    skos:prefLabel "Item I183"@en-AU ;
    dcat:accessURL <https://www.legislation.gov.au/F2021L00308/2023-08-04/2023-08-04/text/original/epub/OEBPS/document_1/document_1.html#_Toc143604892> ;
    dcat:landingPage "https://www.legislation.gov.au/F2021L00308/2023-08-04/2023-08-04/text/original/epub/OEBPS/document_1/document_1.html#_Toc143604892"^^xsd:anyURI ;
    dcat:theme legcons:Item .

F2021L00308:184 a legcons:Item,
        owl:Class,
        dcat:Resource ;
    rdfs:label "Item - I184 8 14  Official markEuropean Union"@en-AU ;
    dct:isPartOf F2021L00308:177 ;
    dct:isReferencedBy F2021L00308: ;
    rdfs:comment "8 14  Official markEuropean Union - Abrievated Graph Key: I184"@en-AU ;
    skos:definition "8 14  Official markEuropean Union"@en-AU ;
    skos:narrower F2021L00308:177 ;
    skos:prefLabel "Item I184"@en-AU ;
    dcat:accessURL <https://www.legislation.gov.au/F2021L00308/2023-08-04/2023-08-04/text/original/epub/OEBPS/document_1/document_1.html#_Toc143604893> ;
    dcat:landingPage "https://www.legislation.gov.au/F2021L00308/2023-08-04/2023-08-04/text/original/epub/OEBPS/document_1/document_1.html#_Toc143604893"^^xsd:anyURI ;
    dcat:theme legcons:Item .

F2021L00308:185 a legcons:Item,
        owl:Class,
        dcat:Resource ;
    rdfs:label "Item - I185 8 15  Official markcarton seal"@en-AU ;
    dct:isPartOf F2021L00308:177 ;
    dct:isReferencedBy F2021L00308: ;
    rdfs:comment "8 15  Official markcarton seal - Abrievated Graph Key: I185"@en-AU ;
    skos:definition "8 15  Official markcarton seal"@en-AU ;
    skos:narrower F2021L00308:177 ;
    skos:prefLabel "Item I185"@en-AU ;
    dcat:accessURL <https://www.legislation.gov.au/F2021L00308/2023-08-04/2023-08-04/text/original/epub/OEBPS/document_1/document_1.html#_Toc143604894> ;
    dcat:landingPage "https://www.legislation.gov.au/F2021L00308/2023-08-04/2023-08-04/text/original/epub/OEBPS/document_1/document_1.html#_Toc143604894"^^xsd:anyURI ;
    dcat:theme legcons:Item .

F2021L00308:186 a legcons:Item,
        owl:Class,
        dcat:Resource ;
    rdfs:label "Item - I186 8 16  Official markcarton seal rabbit meat ratite meat rabbit meat products or ratite meat products opened for assessment and resealed"@en-AU ;
    dct:isPartOf F2021L00308:177 ;
    dct:isReferencedBy F2021L00308: ;
    rdfs:comment "8 16  Official markcarton seal rabbit meat ratite meat rabbit meat products or ratite meat products opened for assessment and resealed - Abrievated Graph Key: I186"@en-AU ;
    skos:definition "8 16  Official markcarton seal rabbit meat ratite meat rabbit meat products or ratite meat products opened for assessment and resealed"@en-AU ;
    skos:narrower F2021L00308:177 ;
    skos:prefLabel "Item I186"@en-AU ;
    dcat:accessURL <https://www.legislation.gov.au/F2021L00308/2023-08-04/2023-08-04/text/original/epub/OEBPS/document_1/document_1.html#_Toc143604895> ;
    dcat:landingPage "https://www.legislation.gov.au/F2021L00308/2023-08-04/2023-08-04/text/original/epub/OEBPS/document_1/document_1.html#_Toc143604895"^^xsd:anyURI ;
    dcat:theme legcons:Item .

F2021L00308:187 a legcons:Item,
        owl:Class,
        dcat:Resource ;
    rdfs:label "Item - I187 8 17  Official markAustralian Government"@en-AU ;
    dct:isPartOf F2021L00308:177 ;
    dct:isReferencedBy F2021L00308: ;
    rdfs:comment "8 17  Official markAustralian Government - Abrievated Graph Key: I187"@en-AU ;
    skos:definition "8 17  Official markAustralian Government"@en-AU ;
    skos:narrower F2021L00308:177 ;
    skos:prefLabel "Item I187"@en-AU ;
    dcat:accessURL <https://www.legislation.gov.au/F2021L00308/2023-08-04/2023-08-04/text/original/epub/OEBPS/document_1/document_1.html#_Toc143604896> ;
    dcat:landingPage "https://www.legislation.gov.au/F2021L00308/2023-08-04/2023-08-04/text/original/epub/OEBPS/document_1/document_1.html#_Toc143604896"^^xsd:anyURI ;
    dcat:theme legcons:Item .

F2021L00308:189 a legcons:Item,
        owl:Class,
        dcat:Resource ;
    rdfs:label "Item - I189 8 18  Purpose and application of this Division"@en-AU ;
    dct:isPartOf F2021L00308:188 ;
    dct:isReferencedBy F2021L00308: ;
    rdfs:comment "8 18  Purpose and application of this Division - Abrievated Graph Key: I189"@en-AU ;
    skos:definition "8 18  Purpose and application of this Division"@en-AU ;
    skos:narrower F2021L00308:188 ;
    skos:prefLabel "Item I189"@en-AU ;
    dcat:accessURL <https://www.legislation.gov.au/F2021L00308/2023-08-04/2023-08-04/text/original/epub/OEBPS/document_1/document_1.html#_Toc143604898> ;
    dcat:landingPage "https://www.legislation.gov.au/F2021L00308/2023-08-04/2023-08-04/text/original/epub/OEBPS/document_1/document_1.html#_Toc143604898"^^xsd:anyURI ;
    dcat:theme legcons:Item .

F2021L00308:190 a legcons:Item,
        owl:Class,
        dcat:Resource ;
    rdfs:label "Item - I190 8 19  Interpretation"@en-AU ;
    dct:isPartOf F2021L00308:188 ;
    dct:isReferencedBy F2021L00308: ;
    rdfs:comment "8 19  Interpretation - Abrievated Graph Key: I190"@en-AU ;
    skos:definition "8 19  Interpretation"@en-AU ;
    skos:narrower F2021L00308:188 ;
    skos:prefLabel "Item I190"@en-AU ;
    dcat:accessURL <https://www.legislation.gov.au/F2021L00308/2023-08-04/2023-08-04/text/original/epub/OEBPS/document_1/document_1.html#_Toc143604899> ;
    dcat:landingPage "https://www.legislation.gov.au/F2021L00308/2023-08-04/2023-08-04/text/original/epub/OEBPS/document_1/document_1.html#_Toc143604899"^^xsd:anyURI ;
    dcat:theme legcons:Item .

F2021L00308:191 a legcons:Item,
        owl:Class,
        dcat:Resource ;
    rdfs:label "Item - I191 8 20  Persons who may manufacture or supply official marks for rabbit meat ratite meat rabbit meat products or ratite meat products"@en-AU ;
    dct:isPartOf F2021L00308:188 ;
    dct:isReferencedBy F2021L00308: ;
    rdfs:comment "8 20  Persons who may manufacture or supply official marks for rabbit meat ratite meat rabbit meat products or ratite meat products - Abrievated Graph Key: I191"@en-AU ;
    skos:definition "8 20  Persons who may manufacture or supply official marks for rabbit meat ratite meat rabbit meat products or ratite meat products"@en-AU ;
    skos:narrower F2021L00308:188 ;
    skos:prefLabel "Item I191"@en-AU ;
    dcat:accessURL <https://www.legislation.gov.au/F2021L00308/2023-08-04/2023-08-04/text/original/epub/OEBPS/document_1/document_1.html#_Toc143604900> ;
    dcat:landingPage "https://www.legislation.gov.au/F2021L00308/2023-08-04/2023-08-04/text/original/epub/OEBPS/document_1/document_1.html#_Toc143604900"^^xsd:anyURI ;
    dcat:theme legcons:Item .

F2021L00308:192 a legcons:Item,
        owl:Class,
        dcat:Resource ;
    rdfs:label "Item - I192 8 21  Persons who may possess official marks that have not been applied to rabbit meat ratite meat rabbit meat products or ratite meat products"@en-AU ;
    dct:isPartOf F2021L00308:188 ;
    dct:isReferencedBy F2021L00308: ;
    rdfs:comment "8 21  Persons who may possess official marks that have not been applied to rabbit meat ratite meat rabbit meat products or ratite meat products - Abrievated Graph Key: I192"@en-AU ;
    skos:definition "8 21  Persons who may possess official marks that have not been applied to rabbit meat ratite meat rabbit meat products or ratite meat products"@en-AU ;
    skos:narrower F2021L00308:188 ;
    skos:prefLabel "Item I192"@en-AU ;
    dcat:accessURL <https://www.legislation.gov.au/F2021L00308/2023-08-04/2023-08-04/text/original/epub/OEBPS/document_1/document_1.html#_Toc143604901> ;
    dcat:landingPage "https://www.legislation.gov.au/F2021L00308/2023-08-04/2023-08-04/text/original/epub/OEBPS/document_1/document_1.html#_Toc143604901"^^xsd:anyURI ;
    dcat:theme legcons:Item .

F2021L00308:193 a legcons:Item,
        owl:Class,
        dcat:Resource ;
    rdfs:label "Item - I193 8 22  Persons who may apply official marks to rabbit meat ratite meat rabbit meat products or ratite meat products etc"@en-AU ;
    dct:isPartOf F2021L00308:188 ;
    dct:isReferencedBy F2021L00308: ;
    rdfs:comment "8 22  Persons who may apply official marks to rabbit meat ratite meat rabbit meat products or ratite meat products etc - Abrievated Graph Key: I193"@en-AU ;
    skos:definition "8 22  Persons who may apply official marks to rabbit meat ratite meat rabbit meat products or ratite meat products etc"@en-AU ;
    skos:narrower F2021L00308:188 ;
    skos:prefLabel "Item I193"@en-AU ;
    dcat:accessURL <https://www.legislation.gov.au/F2021L00308/2023-08-04/2023-08-04/text/original/epub/OEBPS/document_1/document_1.html#_Toc143604902> ;
    dcat:landingPage "https://www.legislation.gov.au/F2021L00308/2023-08-04/2023-08-04/text/original/epub/OEBPS/document_1/document_1.html#_Toc143604902"^^xsd:anyURI ;
    dcat:theme legcons:Item .

F2021L00308:194 a legcons:Item,
        owl:Class,
        dcat:Resource ;
    rdfs:label "Item - I194 8 23  Circumstances in which official mark must not be applied to rabbit meat ratite meat rabbit meat products or ratite meat products"@en-AU ;
    dct:isPartOf F2021L00308:188 ;
    dct:isReferencedBy F2021L00308: ;
    rdfs:comment "8 23  Circumstances in which official mark must not be applied to rabbit meat ratite meat rabbit meat products or ratite meat products - Abrievated Graph Key: I194"@en-AU ;
    skos:definition "8 23  Circumstances in which official mark must not be applied to rabbit meat ratite meat rabbit meat products or ratite meat products"@en-AU ;
    skos:narrower F2021L00308:188 ;
    skos:prefLabel "Item I194"@en-AU ;
    dcat:accessURL <https://www.legislation.gov.au/F2021L00308/2023-08-04/2023-08-04/text/original/epub/OEBPS/document_1/document_1.html#_Toc143604903> ;
    dcat:landingPage "https://www.legislation.gov.au/F2021L00308/2023-08-04/2023-08-04/text/original/epub/OEBPS/document_1/document_1.html#_Toc143604903"^^xsd:anyURI ;
    dcat:theme legcons:Item .

F2021L00308:195 a legcons:Item,
        owl:Class,
        dcat:Resource ;
    rdfs:label "Item - I195 8 24  Alteration of and interference with official marks"@en-AU ;
    dct:isPartOf F2021L00308:188 ;
    dct:isReferencedBy F2021L00308: ;
    rdfs:comment "8 24  Alteration of and interference with official marks - Abrievated Graph Key: I195"@en-AU ;
    skos:definition "8 24  Alteration of and interference with official marks"@en-AU ;
    skos:narrower F2021L00308:188 ;
    skos:prefLabel "Item I195"@en-AU ;
    dcat:accessURL <https://www.legislation.gov.au/F2021L00308/2023-08-04/2023-08-04/text/original/epub/OEBPS/document_1/document_1.html#_Toc143604904> ;
    dcat:landingPage "https://www.legislation.gov.au/F2021L00308/2023-08-04/2023-08-04/text/original/epub/OEBPS/document_1/document_1.html#_Toc143604904"^^xsd:anyURI ;
    dcat:theme legcons:Item .

F2021L00308:196 a legcons:Item,
        owl:Class,
        dcat:Resource ;
    rdfs:label "Item - I196 8 25  Official marks must be legible and securely attached"@en-AU ;
    dct:isPartOf F2021L00308:188 ;
    dct:isReferencedBy F2021L00308: ;
    rdfs:comment "8 25  Official marks must be legible and securely attached - Abrievated Graph Key: I196"@en-AU ;
    skos:definition "8 25  Official marks must be legible and securely attached"@en-AU ;
    skos:narrower F2021L00308:188 ;
    skos:prefLabel "Item I196"@en-AU ;
    dcat:accessURL <https://www.legislation.gov.au/F2021L00308/2023-08-04/2023-08-04/text/original/epub/OEBPS/document_1/document_1.html#_Toc143604905> ;
    dcat:landingPage "https://www.legislation.gov.au/F2021L00308/2023-08-04/2023-08-04/text/original/epub/OEBPS/document_1/document_1.html#_Toc143604905"^^xsd:anyURI ;
    dcat:theme legcons:Item .

F2021L00308:197 a legcons:Item,
        owl:Class,
        dcat:Resource ;
    rdfs:label "Item - I197 8 26  Security of official marks"@en-AU ;
    dct:isPartOf F2021L00308:188 ;
    dct:isReferencedBy F2021L00308: ;
    rdfs:comment "8 26  Security of official marks - Abrievated Graph Key: I197"@en-AU ;
    skos:definition "8 26  Security of official marks"@en-AU ;
    skos:narrower F2021L00308:188 ;
    skos:prefLabel "Item I197"@en-AU ;
    dcat:accessURL <https://www.legislation.gov.au/F2021L00308/2023-08-04/2023-08-04/text/original/epub/OEBPS/document_1/document_1.html#_Toc143604906> ;
    dcat:landingPage "https://www.legislation.gov.au/F2021L00308/2023-08-04/2023-08-04/text/original/epub/OEBPS/document_1/document_1.html#_Toc143604906"^^xsd:anyURI ;
    dcat:theme legcons:Item .

F2021L00308:198 a legcons:Item,
        owl:Class,
        dcat:Resource ;
    rdfs:label "Item - I198 8 27  Removal or defacement of official marks"@en-AU ;
    dct:isPartOf F2021L00308:188 ;
    dct:isReferencedBy F2021L00308: ;
    rdfs:comment "8 27  Removal or defacement of official marks - Abrievated Graph Key: I198"@en-AU ;
    skos:definition "8 27  Removal or defacement of official marks"@en-AU ;
    skos:narrower F2021L00308:188 ;
    skos:prefLabel "Item I198"@en-AU ;
    dcat:accessURL <https://www.legislation.gov.au/F2021L00308/2023-08-04/2023-08-04/text/original/epub/OEBPS/document_1/document_1.html#_Toc143604907> ;
    dcat:landingPage "https://www.legislation.gov.au/F2021L00308/2023-08-04/2023-08-04/text/original/epub/OEBPS/document_1/document_1.html#_Toc143604907"^^xsd:anyURI ;
    dcat:theme legcons:Item .

F2021L00308:199 a legcons:Item,
        owl:Class,
        dcat:Resource ;
    rdfs:label "Item - I199 8 28  Records of official marks manufactured or supplied"@en-AU ;
    dct:isPartOf F2021L00308:188 ;
    dct:isReferencedBy F2021L00308: ;
    rdfs:comment "8 28  Records of official marks manufactured or supplied - Abrievated Graph Key: I199"@en-AU ;
    skos:definition "8 28  Records of official marks manufactured or supplied"@en-AU ;
    skos:narrower F2021L00308:188 ;
    skos:prefLabel "Item I199"@en-AU ;
    dcat:accessURL <https://www.legislation.gov.au/F2021L00308/2023-08-04/2023-08-04/text/original/epub/OEBPS/document_1/document_1.html#_Toc143604908> ;
    dcat:landingPage "https://www.legislation.gov.au/F2021L00308/2023-08-04/2023-08-04/text/original/epub/OEBPS/document_1/document_1.html#_Toc143604908"^^xsd:anyURI ;
    dcat:theme legcons:Item .

F2021L00308:2 a legcons:Part,
        owl:Class,
        dcat:Resource ;
    rdfs:label "Part - P2 Part 1 Preliminary"@en-AU ;
    dct:isPartOf F2021L00308:1 ;
    dct:isReferencedBy F2021L00308: ;
    rdfs:comment "Part 1 Preliminary - Abrievated Graph Key: P2"@en-AU ;
    skos:definition "Part 1 Preliminary"@en-AU ;
    skos:narrower F2021L00308:1 ;
    skos:prefLabel "Part P2"@en-AU ;
    dcat:accessURL <https://www.legislation.gov.au/F2021L00308/2023-08-04/2023-08-04/text/original/epub/OEBPS/document_1/document_1.html#_Toc143604711> ;
    dcat:landingPage "https://www.legislation.gov.au/F2021L00308/2023-08-04/2023-08-04/text/original/epub/OEBPS/document_1/document_1.html#_Toc143604711"^^xsd:anyURI ;
    dcat:theme legcons:Part .

F2021L00308:20 a legcons:Item,
        owl:Class,
        dcat:Resource ;
    rdfs:label "Item - I20 2 3  Purpose and application of this Division"@en-AU ;
    dct:isPartOf F2021L00308:19 ;
    dct:isReferencedBy F2021L00308: ;
    rdfs:comment "2 3  Purpose and application of this Division - Abrievated Graph Key: I20"@en-AU ;
    skos:definition "2 3  Purpose and application of this Division"@en-AU ;
    skos:narrower F2021L00308:19 ;
    skos:prefLabel "Item I20"@en-AU ;
    dcat:accessURL <https://www.legislation.gov.au/F2021L00308/2023-08-04/2023-08-04/text/original/epub/OEBPS/document_1/document_1.html#_Toc143604729> ;
    dcat:landingPage "https://www.legislation.gov.au/F2021L00308/2023-08-04/2023-08-04/text/original/epub/OEBPS/document_1/document_1.html#_Toc143604729"^^xsd:anyURI ;
    dcat:theme legcons:Item .

F2021L00308:200 a legcons:Item,
        owl:Class,
        dcat:Resource ;
    rdfs:label "Item - I200 8 29  Records of official marks received applied removed defaced destroyed or returned"@en-AU ;
    dct:isPartOf F2021L00308:188 ;
    dct:isReferencedBy F2021L00308: ;
    rdfs:comment "8 29  Records of official marks received applied removed defaced destroyed or returned - Abrievated Graph Key: I200"@en-AU ;
    skos:definition "8 29  Records of official marks received applied removed defaced destroyed or returned"@en-AU ;
    skos:narrower F2021L00308:188 ;
    skos:prefLabel "Item I200"@en-AU ;
    dcat:accessURL <https://www.legislation.gov.au/F2021L00308/2023-08-04/2023-08-04/text/original/epub/OEBPS/document_1/document_1.html#_Toc143604909> ;
    dcat:landingPage "https://www.legislation.gov.au/F2021L00308/2023-08-04/2023-08-04/text/original/epub/OEBPS/document_1/document_1.html#_Toc143604909"^^xsd:anyURI ;
    dcat:theme legcons:Item .

F2021L00308:202 a legcons:Item,
        owl:Class,
        dcat:Resource ;
    rdfs:label "Item - I202 8 30  Purpose of this Division"@en-AU ;
    dct:isPartOf F2021L00308:201 ;
    dct:isReferencedBy F2021L00308: ;
    rdfs:comment "8 30  Purpose of this Division - Abrievated Graph Key: I202"@en-AU ;
    skos:definition "8 30  Purpose of this Division"@en-AU ;
    skos:narrower F2021L00308:201 ;
    skos:prefLabel "Item I202"@en-AU ;
    dcat:accessURL <https://www.legislation.gov.au/F2021L00308/2023-08-04/2023-08-04/text/original/epub/OEBPS/document_1/document_1.html#_Toc143604911> ;
    dcat:landingPage "https://www.legislation.gov.au/F2021L00308/2023-08-04/2023-08-04/text/original/epub/OEBPS/document_1/document_1.html#_Toc143604911"^^xsd:anyURI ;
    dcat:theme legcons:Item .

F2021L00308:203 a legcons:Item,
        owl:Class,
        dcat:Resource ;
    rdfs:label "Item - I203 8 31  Circumstances in which a mark resembles an official mark"@en-AU ;
    dct:isPartOf F2021L00308:201 ;
    dct:isReferencedBy F2021L00308: ;
    rdfs:comment "8 31  Circumstances in which a mark resembles an official mark - Abrievated Graph Key: I203"@en-AU ;
    skos:definition "8 31  Circumstances in which a mark resembles an official mark"@en-AU ;
    skos:narrower F2021L00308:201 ;
    skos:prefLabel "Item I203"@en-AU ;
    dcat:accessURL <https://www.legislation.gov.au/F2021L00308/2023-08-04/2023-08-04/text/original/epub/OEBPS/document_1/document_1.html#_Toc143604912> ;
    dcat:landingPage "https://www.legislation.gov.au/F2021L00308/2023-08-04/2023-08-04/text/original/epub/OEBPS/document_1/document_1.html#_Toc143604912"^^xsd:anyURI ;
    dcat:theme legcons:Item .

F2021L00308:204 a legcons:Item,
        owl:Class,
        dcat:Resource ;
    rdfs:label "Item - I204 8 32  Persons who may apply a resemblance"@en-AU ;
    dct:isPartOf F2021L00308:201 ;
    dct:isReferencedBy F2021L00308: ;
    rdfs:comment "8 32  Persons who may apply a resemblance - Abrievated Graph Key: I204"@en-AU ;
    skos:definition "8 32  Persons who may apply a resemblance"@en-AU ;
    skos:narrower F2021L00308:201 ;
    skos:prefLabel "Item I204"@en-AU ;
    dcat:accessURL <https://www.legislation.gov.au/F2021L00308/2023-08-04/2023-08-04/text/original/epub/OEBPS/document_1/document_1.html#_Toc143604913> ;
    dcat:landingPage "https://www.legislation.gov.au/F2021L00308/2023-08-04/2023-08-04/text/original/epub/OEBPS/document_1/document_1.html#_Toc143604913"^^xsd:anyURI ;
    dcat:theme legcons:Item .

F2021L00308:206 a legcons:Item,
        owl:Class,
        dcat:Resource ;
    rdfs:label "Item - I206 8 33  Purpose of this Division"@en-AU ;
    dct:isPartOf F2021L00308:205 ;
    dct:isReferencedBy F2021L00308: ;
    rdfs:comment "8 33  Purpose of this Division - Abrievated Graph Key: I206"@en-AU ;
    skos:definition "8 33  Purpose of this Division"@en-AU ;
    skos:narrower F2021L00308:205 ;
    skos:prefLabel "Item I206"@en-AU ;
    dcat:accessURL <https://www.legislation.gov.au/F2021L00308/2023-08-04/2023-08-04/text/original/epub/OEBPS/document_1/document_1.html#_Toc143604915> ;
    dcat:landingPage "https://www.legislation.gov.au/F2021L00308/2023-08-04/2023-08-04/text/original/epub/OEBPS/document_1/document_1.html#_Toc143604915"^^xsd:anyURI ;
    dcat:theme legcons:Item .

F2021L00308:207 a legcons:Item,
        owl:Class,
        dcat:Resource ;
    rdfs:label "Item - I207 8 34  Persons who may manufacture supply or possess official marking devices"@en-AU ;
    dct:isPartOf F2021L00308:205 ;
    dct:isReferencedBy F2021L00308: ;
    rdfs:comment "8 34  Persons who may manufacture supply or possess official marking devices - Abrievated Graph Key: I207"@en-AU ;
    skos:definition "8 34  Persons who may manufacture supply or possess official marking devices"@en-AU ;
    skos:narrower F2021L00308:205 ;
    skos:prefLabel "Item I207"@en-AU ;
    dcat:accessURL <https://www.legislation.gov.au/F2021L00308/2023-08-04/2023-08-04/text/original/epub/OEBPS/document_1/document_1.html#_Toc143604916> ;
    dcat:landingPage "https://www.legislation.gov.au/F2021L00308/2023-08-04/2023-08-04/text/original/epub/OEBPS/document_1/document_1.html#_Toc143604916"^^xsd:anyURI ;
    dcat:theme legcons:Item .

F2021L00308:208 a legcons:Item,
        owl:Class,
        dcat:Resource ;
    rdfs:label "Item - I208 8 35  Security of official marking devices"@en-AU ;
    dct:isPartOf F2021L00308:205 ;
    dct:isReferencedBy F2021L00308: ;
    rdfs:comment "8 35  Security of official marking devices - Abrievated Graph Key: I208"@en-AU ;
    skos:definition "8 35  Security of official marking devices"@en-AU ;
    skos:narrower F2021L00308:205 ;
    skos:prefLabel "Item I208"@en-AU ;
    dcat:accessURL <https://www.legislation.gov.au/F2021L00308/2023-08-04/2023-08-04/text/original/epub/OEBPS/document_1/document_1.html#_Toc143604917> ;
    dcat:landingPage "https://www.legislation.gov.au/F2021L00308/2023-08-04/2023-08-04/text/original/epub/OEBPS/document_1/document_1.html#_Toc143604917"^^xsd:anyURI ;
    dcat:theme legcons:Item .

F2021L00308:209 a legcons:Item,
        owl:Class,
        dcat:Resource ;
    rdfs:label "Item - I209 8 36  Damaged etc official marking devices"@en-AU ;
    dct:isPartOf F2021L00308:205 ;
    dct:isReferencedBy F2021L00308: ;
    rdfs:comment "8 36  Damaged etc official marking devices - Abrievated Graph Key: I209"@en-AU ;
    skos:definition "8 36  Damaged etc official marking devices"@en-AU ;
    skos:narrower F2021L00308:205 ;
    skos:prefLabel "Item I209"@en-AU ;
    dcat:accessURL <https://www.legislation.gov.au/F2021L00308/2023-08-04/2023-08-04/text/original/epub/OEBPS/document_1/document_1.html#_Toc143604918> ;
    dcat:landingPage "https://www.legislation.gov.au/F2021L00308/2023-08-04/2023-08-04/text/original/epub/OEBPS/document_1/document_1.html#_Toc143604918"^^xsd:anyURI ;
    dcat:theme legcons:Item .

F2021L00308:21 a legcons:Item,
        owl:Class,
        dcat:Resource ;
    rdfs:label "Item - I21 2 4  Export of prescribed rabbit meat ratite meat rabbit meat products or ratite meat products is prohibited unless prescribed conditions are complied with"@en-AU ;
    dct:isPartOf F2021L00308:19 ;
    dct:isReferencedBy F2021L00308: ;
    rdfs:comment "2 4  Export of prescribed rabbit meat ratite meat rabbit meat products or ratite meat products is prohibited unless prescribed conditions are complied with - Abrievated Graph Key: I21"@en-AU ;
    skos:definition "2 4  Export of prescribed rabbit meat ratite meat rabbit meat products or ratite meat products is prohibited unless prescribed conditions are complied with"@en-AU ;
    skos:narrower F2021L00308:19 ;
    skos:prefLabel "Item I21"@en-AU ;
    dcat:accessURL <https://www.legislation.gov.au/F2021L00308/2023-08-04/2023-08-04/text/original/epub/OEBPS/document_1/document_1.html#_Toc143604730> ;
    dcat:landingPage "https://www.legislation.gov.au/F2021L00308/2023-08-04/2023-08-04/text/original/epub/OEBPS/document_1/document_1.html#_Toc143604730"^^xsd:anyURI ;
    dcat:theme legcons:Item .

F2021L00308:210 a legcons:Item,
        owl:Class,
        dcat:Resource ;
    rdfs:label "Item - I210 8 37  Records of official marking devices manufactured or supplied"@en-AU ;
    dct:isPartOf F2021L00308:205 ;
    dct:isReferencedBy F2021L00308: ;
    rdfs:comment "8 37  Records of official marking devices manufactured or supplied - Abrievated Graph Key: I210"@en-AU ;
    skos:definition "8 37  Records of official marking devices manufactured or supplied"@en-AU ;
    skos:narrower F2021L00308:205 ;
    skos:prefLabel "Item I210"@en-AU ;
    dcat:accessURL <https://www.legislation.gov.au/F2021L00308/2023-08-04/2023-08-04/text/original/epub/OEBPS/document_1/document_1.html#_Toc143604919> ;
    dcat:landingPage "https://www.legislation.gov.au/F2021L00308/2023-08-04/2023-08-04/text/original/epub/OEBPS/document_1/document_1.html#_Toc143604919"^^xsd:anyURI ;
    dcat:theme legcons:Item .

F2021L00308:211 a legcons:Item,
        owl:Class,
        dcat:Resource ;
    rdfs:label "Item - I211 8 38  Records of official marking devices received used damaged destroyed or returned"@en-AU ;
    dct:isPartOf F2021L00308:205 ;
    dct:isReferencedBy F2021L00308: ;
    rdfs:comment "8 38  Records of official marking devices received used damaged destroyed or returned - Abrievated Graph Key: I211"@en-AU ;
    skos:definition "8 38  Records of official marking devices received used damaged destroyed or returned"@en-AU ;
    skos:narrower F2021L00308:205 ;
    skos:prefLabel "Item I211"@en-AU ;
    dcat:accessURL <https://www.legislation.gov.au/F2021L00308/2023-08-04/2023-08-04/text/original/epub/OEBPS/document_1/document_1.html#_Toc143604920> ;
    dcat:landingPage "https://www.legislation.gov.au/F2021L00308/2023-08-04/2023-08-04/text/original/epub/OEBPS/document_1/document_1.html#_Toc143604920"^^xsd:anyURI ;
    dcat:theme legcons:Item .

F2021L00308:215 a legcons:Item,
        owl:Class,
        dcat:Resource ;
    rdfs:label "Item - I215 9 1  References to audit in this Part"@en-AU ;
    dct:isPartOf F2021L00308:214 ;
    dct:isReferencedBy F2021L00308: ;
    rdfs:comment "9 1  References to audit in this Part - Abrievated Graph Key: I215"@en-AU ;
    skos:definition "9 1  References to audit in this Part"@en-AU ;
    skos:narrower F2021L00308:214 ;
    skos:prefLabel "Item I215"@en-AU ;
    dcat:accessURL <https://www.legislation.gov.au/F2021L00308/2023-08-04/2023-08-04/text/original/epub/OEBPS/document_1/document_1.html#_Toc143604924> ;
    dcat:landingPage "https://www.legislation.gov.au/F2021L00308/2023-08-04/2023-08-04/text/original/epub/OEBPS/document_1/document_1.html#_Toc143604924"^^xsd:anyURI ;
    dcat:theme legcons:Item .

F2021L00308:217 a legcons:Item,
        owl:Class,
        dcat:Resource ;
    rdfs:label "Item - I217 9 2  Purpose of this Division"@en-AU ;
    dct:isPartOf F2021L00308:216 ;
    dct:isReferencedBy F2021L00308: ;
    rdfs:comment "9 2  Purpose of this Division - Abrievated Graph Key: I217"@en-AU ;
    skos:definition "9 2  Purpose of this Division"@en-AU ;
    skos:narrower F2021L00308:216 ;
    skos:prefLabel "Item I217"@en-AU ;
    dcat:accessURL <https://www.legislation.gov.au/F2021L00308/2023-08-04/2023-08-04/text/original/epub/OEBPS/document_1/document_1.html#_Toc143604926> ;
    dcat:landingPage "https://www.legislation.gov.au/F2021L00308/2023-08-04/2023-08-04/text/original/epub/OEBPS/document_1/document_1.html#_Toc143604926"^^xsd:anyURI ;
    dcat:theme legcons:Item .

F2021L00308:218 a legcons:Item,
        owl:Class,
        dcat:Resource ;
    rdfs:label "Item - I218 9 3  Manner in which audit must be conducted"@en-AU ;
    dct:isPartOf F2021L00308:216 ;
    dct:isReferencedBy F2021L00308: ;
    rdfs:comment "9 3  Manner in which audit must be conducted - Abrievated Graph Key: I218"@en-AU ;
    skos:definition "9 3  Manner in which audit must be conducted"@en-AU ;
    skos:narrower F2021L00308:216 ;
    skos:prefLabel "Item I218"@en-AU ;
    dcat:accessURL <https://www.legislation.gov.au/F2021L00308/2023-08-04/2023-08-04/text/original/epub/OEBPS/document_1/document_1.html#_Toc143604927> ;
    dcat:landingPage "https://www.legislation.gov.au/F2021L00308/2023-08-04/2023-08-04/text/original/epub/OEBPS/document_1/document_1.html#_Toc143604927"^^xsd:anyURI ;
    dcat:theme legcons:Item .

F2021L00308:219 a legcons:Item,
        owl:Class,
        dcat:Resource ;
    rdfs:label "Item - I219 9 4  Notice of non compliance with requirements"@en-AU ;
    dct:isPartOf F2021L00308:216 ;
    dct:isReferencedBy F2021L00308: ;
    rdfs:comment "9 4  Notice of non compliance with requirements - Abrievated Graph Key: I219"@en-AU ;
    skos:definition "9 4  Notice of non compliance with requirements"@en-AU ;
    skos:narrower F2021L00308:216 ;
    skos:prefLabel "Item I219"@en-AU ;
    dcat:accessURL <https://www.legislation.gov.au/F2021L00308/2023-08-04/2023-08-04/text/original/epub/OEBPS/document_1/document_1.html#_Toc143604928> ;
    dcat:landingPage "https://www.legislation.gov.au/F2021L00308/2023-08-04/2023-08-04/text/original/epub/OEBPS/document_1/document_1.html#_Toc143604928"^^xsd:anyURI ;
    dcat:theme legcons:Item .

F2021L00308:220 a legcons:Item,
        owl:Class,
        dcat:Resource ;
    rdfs:label "Item - I220 9 5  Audit reports"@en-AU ;
    dct:isPartOf F2021L00308:216 ;
    dct:isReferencedBy F2021L00308: ;
    rdfs:comment "9 5  Audit reports - Abrievated Graph Key: I220"@en-AU ;
    skos:definition "9 5  Audit reports"@en-AU ;
    skos:narrower F2021L00308:216 ;
    skos:prefLabel "Item I220"@en-AU ;
    dcat:accessURL <https://www.legislation.gov.au/F2021L00308/2023-08-04/2023-08-04/text/original/epub/OEBPS/document_1/document_1.html#_Toc143604929> ;
    dcat:landingPage "https://www.legislation.gov.au/F2021L00308/2023-08-04/2023-08-04/text/original/epub/OEBPS/document_1/document_1.html#_Toc143604929"^^xsd:anyURI ;
    dcat:theme legcons:Item .

F2021L00308:222 a legcons:Item,
        owl:Class,
        dcat:Resource ;
    rdfs:label "Item - I222 9 6  Purpose of this Division"@en-AU ;
    dct:isPartOf F2021L00308:221 ;
    dct:isReferencedBy F2021L00308: ;
    rdfs:comment "9 6  Purpose of this Division - Abrievated Graph Key: I222"@en-AU ;
    skos:definition "9 6  Purpose of this Division"@en-AU ;
    skos:narrower F2021L00308:221 ;
    skos:prefLabel "Item I222"@en-AU ;
    dcat:accessURL <https://www.legislation.gov.au/F2021L00308/2023-08-04/2023-08-04/text/original/epub/OEBPS/document_1/document_1.html#_Toc143604931> ;
    dcat:landingPage "https://www.legislation.gov.au/F2021L00308/2023-08-04/2023-08-04/text/original/epub/OEBPS/document_1/document_1.html#_Toc143604931"^^xsd:anyURI ;
    dcat:theme legcons:Item .

F2021L00308:223 a legcons:Item,
        owl:Class,
        dcat:Resource ;
    rdfs:label "Item - I223 9 7  Application for approval"@en-AU ;
    dct:isPartOf F2021L00308:221 ;
    dct:isReferencedBy F2021L00308: ;
    rdfs:comment "9 7  Application for approval - Abrievated Graph Key: I223"@en-AU ;
    skos:definition "9 7  Application for approval"@en-AU ;
    skos:narrower F2021L00308:221 ;
    skos:prefLabel "Item I223"@en-AU ;
    dcat:accessURL <https://www.legislation.gov.au/F2021L00308/2023-08-04/2023-08-04/text/original/epub/OEBPS/document_1/document_1.html#_Toc143604932> ;
    dcat:landingPage "https://www.legislation.gov.au/F2021L00308/2023-08-04/2023-08-04/text/original/epub/OEBPS/document_1/document_1.html#_Toc143604932"^^xsd:anyURI ;
    dcat:theme legcons:Item .

F2021L00308:224 a legcons:Item,
        owl:Class,
        dcat:Resource ;
    rdfs:label "Item - I224 9 8  Secretary must decide whether to approve applicant to conduct audits"@en-AU ;
    dct:isPartOf F2021L00308:221 ;
    dct:isReferencedBy F2021L00308: ;
    rdfs:comment "9 8  Secretary must decide whether to approve applicant to conduct audits - Abrievated Graph Key: I224"@en-AU ;
    skos:definition "9 8  Secretary must decide whether to approve applicant to conduct audits"@en-AU ;
    skos:narrower F2021L00308:221 ;
    skos:prefLabel "Item I224"@en-AU ;
    dcat:accessURL <https://www.legislation.gov.au/F2021L00308/2023-08-04/2023-08-04/text/original/epub/OEBPS/document_1/document_1.html#_Toc143604933> ;
    dcat:landingPage "https://www.legislation.gov.au/F2021L00308/2023-08-04/2023-08-04/text/original/epub/OEBPS/document_1/document_1.html#_Toc143604933"^^xsd:anyURI ;
    dcat:theme legcons:Item .

F2021L00308:225 a legcons:Item,
        owl:Class,
        dcat:Resource ;
    rdfs:label "Item - I225 9 9  Dealing with applications"@en-AU ;
    dct:isPartOf F2021L00308:221 ;
    dct:isReferencedBy F2021L00308: ;
    rdfs:comment "9 9  Dealing with applications - Abrievated Graph Key: I225"@en-AU ;
    skos:definition "9 9  Dealing with applications"@en-AU ;
    skos:narrower F2021L00308:221 ;
    skos:prefLabel "Item I225"@en-AU ;
    dcat:accessURL <https://www.legislation.gov.au/F2021L00308/2023-08-04/2023-08-04/text/original/epub/OEBPS/document_1/document_1.html#_Toc143604934> ;
    dcat:landingPage "https://www.legislation.gov.au/F2021L00308/2023-08-04/2023-08-04/text/original/epub/OEBPS/document_1/document_1.html#_Toc143604934"^^xsd:anyURI ;
    dcat:theme legcons:Item .

F2021L00308:226 a legcons:Item,
        owl:Class,
        dcat:Resource ;
    rdfs:label "Item - I226 9 10  Conditions of approval"@en-AU ;
    dct:isPartOf F2021L00308:221 ;
    dct:isReferencedBy F2021L00308: ;
    rdfs:comment "9 10  Conditions of approval - Abrievated Graph Key: I226"@en-AU ;
    skos:definition "9 10  Conditions of approval"@en-AU ;
    skos:narrower F2021L00308:221 ;
    skos:prefLabel "Item I226"@en-AU ;
    dcat:accessURL <https://www.legislation.gov.au/F2021L00308/2023-08-04/2023-08-04/text/original/epub/OEBPS/document_1/document_1.html#_Toc143604935> ;
    dcat:landingPage "https://www.legislation.gov.au/F2021L00308/2023-08-04/2023-08-04/text/original/epub/OEBPS/document_1/document_1.html#_Toc143604935"^^xsd:anyURI ;
    dcat:theme legcons:Item .

F2021L00308:227 a legcons:Item,
        owl:Class,
        dcat:Resource ;
    rdfs:label "Item - I227 9 11  Notice of decision"@en-AU ;
    dct:isPartOf F2021L00308:221 ;
    dct:isReferencedBy F2021L00308: ;
    rdfs:comment "9 11  Notice of decision - Abrievated Graph Key: I227"@en-AU ;
    skos:definition "9 11  Notice of decision"@en-AU ;
    skos:narrower F2021L00308:221 ;
    skos:prefLabel "Item I227"@en-AU ;
    dcat:accessURL <https://www.legislation.gov.au/F2021L00308/2023-08-04/2023-08-04/text/original/epub/OEBPS/document_1/document_1.html#_Toc143604936> ;
    dcat:landingPage "https://www.legislation.gov.au/F2021L00308/2023-08-04/2023-08-04/text/original/epub/OEBPS/document_1/document_1.html#_Toc143604936"^^xsd:anyURI ;
    dcat:theme legcons:Item .

F2021L00308:228 a legcons:Item,
        owl:Class,
        dcat:Resource ;
    rdfs:label "Item - I228 9 12  Period of effect of approval"@en-AU ;
    dct:isPartOf F2021L00308:221 ;
    dct:isReferencedBy F2021L00308: ;
    rdfs:comment "9 12  Period of effect of approval - Abrievated Graph Key: I228"@en-AU ;
    skos:definition "9 12  Period of effect of approval"@en-AU ;
    skos:narrower F2021L00308:221 ;
    skos:prefLabel "Item I228"@en-AU ;
    dcat:accessURL <https://www.legislation.gov.au/F2021L00308/2023-08-04/2023-08-04/text/original/epub/OEBPS/document_1/document_1.html#_Toc143604937> ;
    dcat:landingPage "https://www.legislation.gov.au/F2021L00308/2023-08-04/2023-08-04/text/original/epub/OEBPS/document_1/document_1.html#_Toc143604937"^^xsd:anyURI ;
    dcat:theme legcons:Item .

F2021L00308:229 a legcons:Item,
        owl:Class,
        dcat:Resource ;
    rdfs:label "Item - I229 9 13  Imposing or varying conditions of approval"@en-AU ;
    dct:isPartOf F2021L00308:221 ;
    dct:isReferencedBy F2021L00308: ;
    rdfs:comment "9 13  Imposing or varying conditions of approval - Abrievated Graph Key: I229"@en-AU ;
    skos:definition "9 13  Imposing or varying conditions of approval"@en-AU ;
    skos:narrower F2021L00308:221 ;
    skos:prefLabel "Item I229"@en-AU ;
    dcat:accessURL <https://www.legislation.gov.au/F2021L00308/2023-08-04/2023-08-04/text/original/epub/OEBPS/document_1/document_1.html#_Toc143604938> ;
    dcat:landingPage "https://www.legislation.gov.au/F2021L00308/2023-08-04/2023-08-04/text/original/epub/OEBPS/document_1/document_1.html#_Toc143604938"^^xsd:anyURI ;
    dcat:theme legcons:Item .

F2021L00308:23 a legcons:Item,
        owl:Class,
        dcat:Resource ;
    rdfs:label "Item - I23 2 5  Application of this Part"@en-AU ;
    dct:isPartOf F2021L00308:22 ;
    dct:isReferencedBy F2021L00308: ;
    rdfs:comment "2 5  Application of this Part - Abrievated Graph Key: I23"@en-AU ;
    skos:definition "2 5  Application of this Part"@en-AU ;
    skos:narrower F2021L00308:22 ;
    skos:prefLabel "Item I23"@en-AU ;
    dcat:accessURL <https://www.legislation.gov.au/F2021L00308/2023-08-04/2023-08-04/text/original/epub/OEBPS/document_1/document_1.html#_Toc143604732> ;
    dcat:landingPage "https://www.legislation.gov.au/F2021L00308/2023-08-04/2023-08-04/text/original/epub/OEBPS/document_1/document_1.html#_Toc143604732"^^xsd:anyURI ;
    dcat:theme legcons:Item .

F2021L00308:230 a legcons:Item,
        owl:Class,
        dcat:Resource ;
    rdfs:label "Item - I230 9 14  Revocation of approval"@en-AU ;
    dct:isPartOf F2021L00308:221 ;
    dct:isReferencedBy F2021L00308: ;
    rdfs:comment "9 14  Revocation of approval - Abrievated Graph Key: I230"@en-AU ;
    skos:definition "9 14  Revocation of approval"@en-AU ;
    skos:narrower F2021L00308:221 ;
    skos:prefLabel "Item I230"@en-AU ;
    dcat:accessURL <https://www.legislation.gov.au/F2021L00308/2023-08-04/2023-08-04/text/original/epub/OEBPS/document_1/document_1.html#_Toc143604939> ;
    dcat:landingPage "https://www.legislation.gov.au/F2021L00308/2023-08-04/2023-08-04/text/original/epub/OEBPS/document_1/document_1.html#_Toc143604939"^^xsd:anyURI ;
    dcat:theme legcons:Item .

F2021L00308:231 a legcons:Item,
        owl:Class,
        dcat:Resource ;
    rdfs:label "Item - I231 9 15  Register of approved auditors"@en-AU ;
    dct:isPartOf F2021L00308:221 ;
    dct:isReferencedBy F2021L00308: ;
    rdfs:comment "9 15  Register of approved auditors - Abrievated Graph Key: I231"@en-AU ;
    skos:definition "9 15  Register of approved auditors"@en-AU ;
    skos:narrower F2021L00308:221 ;
    skos:prefLabel "Item I231"@en-AU ;
    dcat:accessURL <https://www.legislation.gov.au/F2021L00308/2023-08-04/2023-08-04/text/original/epub/OEBPS/document_1/document_1.html#_Toc143604940> ;
    dcat:landingPage "https://www.legislation.gov.au/F2021L00308/2023-08-04/2023-08-04/text/original/epub/OEBPS/document_1/document_1.html#_Toc143604940"^^xsd:anyURI ;
    dcat:theme legcons:Item .

F2021L00308:232 a legcons:Item,
        owl:Class,
        dcat:Resource ;
    rdfs:label "Item - I232 9 16  Fit and proper person test"@en-AU ;
    dct:isPartOf F2021L00308:221 ;
    dct:isReferencedBy F2021L00308: ;
    rdfs:comment "9 16  Fit and proper person test - Abrievated Graph Key: I232"@en-AU ;
    skos:definition "9 16  Fit and proper person test"@en-AU ;
    skos:narrower F2021L00308:221 ;
    skos:prefLabel "Item I232"@en-AU ;
    dcat:accessURL <https://www.legislation.gov.au/F2021L00308/2023-08-04/2023-08-04/text/original/epub/OEBPS/document_1/document_1.html#_Toc143604941> ;
    dcat:landingPage "https://www.legislation.gov.au/F2021L00308/2023-08-04/2023-08-04/text/original/epub/OEBPS/document_1/document_1.html#_Toc143604941"^^xsd:anyURI ;
    dcat:theme legcons:Item .

F2021L00308:234 a legcons:Item,
        owl:Class,
        dcat:Resource ;
    rdfs:label "Item - I234 9 17  Circumstances in which assessment may be required or permitted"@en-AU ;
    dct:isPartOf F2021L00308:233 ;
    dct:isReferencedBy F2021L00308: ;
    rdfs:comment "9 17  Circumstances in which assessment may be required or permitted - Abrievated Graph Key: I234"@en-AU ;
    skos:definition "9 17  Circumstances in which assessment may be required or permitted"@en-AU ;
    skos:narrower F2021L00308:233 ;
    skos:prefLabel "Item I234"@en-AU ;
    dcat:accessURL <https://www.legislation.gov.au/F2021L00308/2023-08-04/2023-08-04/text/original/epub/OEBPS/document_1/document_1.html#_Toc143604943> ;
    dcat:landingPage "https://www.legislation.gov.au/F2021L00308/2023-08-04/2023-08-04/text/original/epub/OEBPS/document_1/document_1.html#_Toc143604943"^^xsd:anyURI ;
    dcat:theme legcons:Item .

F2021L00308:236 a legcons:Item,
        owl:Class,
        dcat:Resource ;
    rdfs:label "Item - I236 9 18  Decisions that may be made by operation of computer program"@en-AU ;
    dct:isPartOf F2021L00308:235 ;
    dct:isReferencedBy F2021L00308: ;
    rdfs:comment "9 18  Decisions that may be made by operation of computer program - Abrievated Graph Key: I236"@en-AU ;
    skos:definition "9 18  Decisions that may be made by operation of computer program"@en-AU ;
    skos:narrower F2021L00308:235 ;
    skos:prefLabel "Item I236"@en-AU ;
    dcat:accessURL <https://www.legislation.gov.au/F2021L00308/2023-08-04/2023-08-04/text/original/epub/OEBPS/document_1/document_1.html#_Toc143604945> ;
    dcat:landingPage "https://www.legislation.gov.au/F2021L00308/2023-08-04/2023-08-04/text/original/epub/OEBPS/document_1/document_1.html#_Toc143604945"^^xsd:anyURI ;
    dcat:theme legcons:Item .

F2021L00308:239 a legcons:Item,
        owl:Class,
        dcat:Resource ;
    rdfs:label "Item - I239 9 19  Requirement to be third party authorised officerfit and proper person etc"@en-AU ;
    dct:isPartOf F2021L00308:238 ;
    dct:isReferencedBy F2021L00308: ;
    rdfs:comment "9 19  Requirement to be third party authorised officerfit and proper person etc - Abrievated Graph Key: I239"@en-AU ;
    skos:definition "9 19  Requirement to be third party authorised officerfit and proper person etc"@en-AU ;
    skos:narrower F2021L00308:238 ;
    skos:prefLabel "Item I239"@en-AU ;
    dcat:accessURL <https://www.legislation.gov.au/F2021L00308/2023-08-04/2023-08-04/text/original/epub/OEBPS/document_1/document_1.html#_Toc143604948> ;
    dcat:landingPage "https://www.legislation.gov.au/F2021L00308/2023-08-04/2023-08-04/text/original/epub/OEBPS/document_1/document_1.html#_Toc143604948"^^xsd:anyURI ;
    dcat:theme legcons:Item .

F2021L00308:24 a legcons:Item,
        owl:Class,
        dcat:Resource ;
    rdfs:label "Item - I24 2 6  Period for making application for exemption"@en-AU ;
    dct:isPartOf F2021L00308:22 ;
    dct:isReferencedBy F2021L00308: ;
    rdfs:comment "2 6  Period for making application for exemption - Abrievated Graph Key: I24"@en-AU ;
    skos:definition "2 6  Period for making application for exemption"@en-AU ;
    skos:narrower F2021L00308:22 ;
    skos:prefLabel "Item I24"@en-AU ;
    dcat:accessURL <https://www.legislation.gov.au/F2021L00308/2023-08-04/2023-08-04/text/original/epub/OEBPS/document_1/document_1.html#_Toc143604733> ;
    dcat:landingPage "https://www.legislation.gov.au/F2021L00308/2023-08-04/2023-08-04/text/original/epub/OEBPS/document_1/document_1.html#_Toc143604733"^^xsd:anyURI ;
    dcat:theme legcons:Item .

F2021L00308:241 a legcons:Item,
        owl:Class,
        dcat:Resource ;
    rdfs:label "Item - I241 9 20  Purpose of this Division"@en-AU ;
    dct:isPartOf F2021L00308:240 ;
    dct:isReferencedBy F2021L00308: ;
    rdfs:comment "9 20  Purpose of this Division - Abrievated Graph Key: I241"@en-AU ;
    skos:definition "9 20  Purpose of this Division"@en-AU ;
    skos:narrower F2021L00308:240 ;
    skos:prefLabel "Item I241"@en-AU ;
    dcat:accessURL <https://www.legislation.gov.au/F2021L00308/2023-08-04/2023-08-04/text/original/epub/OEBPS/document_1/document_1.html#_Toc143604950> ;
    dcat:landingPage "https://www.legislation.gov.au/F2021L00308/2023-08-04/2023-08-04/text/original/epub/OEBPS/document_1/document_1.html#_Toc143604950"^^xsd:anyURI ;
    dcat:theme legcons:Item .

F2021L00308:242 a legcons:Item,
        owl:Class,
        dcat:Resource ;
    rdfs:label "Item - I242 9 21  Functions specified in Australian Meat Standard"@en-AU ;
    dct:isPartOf F2021L00308:240 ;
    dct:isReferencedBy F2021L00308: ;
    rdfs:comment "9 21  Functions specified in Australian Meat Standard - Abrievated Graph Key: I242"@en-AU ;
    skos:definition "9 21  Functions specified in Australian Meat Standard"@en-AU ;
    skos:narrower F2021L00308:240 ;
    skos:prefLabel "Item I242"@en-AU ;
    dcat:accessURL <https://www.legislation.gov.au/F2021L00308/2023-08-04/2023-08-04/text/original/epub/OEBPS/document_1/document_1.html#_Toc143604951> ;
    dcat:landingPage "https://www.legislation.gov.au/F2021L00308/2023-08-04/2023-08-04/text/original/epub/OEBPS/document_1/document_1.html#_Toc143604951"^^xsd:anyURI ;
    dcat:theme legcons:Item .

F2021L00308:243 a legcons:Item,
        owl:Class,
        dcat:Resource ;
    rdfs:label "Item - I243 9 22  Applying admission decisions"@en-AU ;
    dct:isPartOf F2021L00308:240 ;
    dct:isReferencedBy F2021L00308: ;
    rdfs:comment "9 22  Applying admission decisions - Abrievated Graph Key: I243"@en-AU ;
    skos:definition "9 22  Applying admission decisions"@en-AU ;
    skos:narrower F2021L00308:240 ;
    skos:prefLabel "Item I243"@en-AU ;
    dcat:accessURL <https://www.legislation.gov.au/F2021L00308/2023-08-04/2023-08-04/text/original/epub/OEBPS/document_1/document_1.html#_Toc143604952> ;
    dcat:landingPage "https://www.legislation.gov.au/F2021L00308/2023-08-04/2023-08-04/text/original/epub/OEBPS/document_1/document_1.html#_Toc143604952"^^xsd:anyURI ;
    dcat:theme legcons:Item .

F2021L00308:244 a legcons:Item,
        owl:Class,
        dcat:Resource ;
    rdfs:label "Item - I244 9 23  Inspections of animals for slaughter and applying ante mortem dispositions"@en-AU ;
    dct:isPartOf F2021L00308:240 ;
    dct:isReferencedBy F2021L00308: ;
    rdfs:comment "9 23  Inspections of animals for slaughter and applying ante mortem dispositions - Abrievated Graph Key: I244"@en-AU ;
    skos:definition "9 23  Inspections of animals for slaughter and applying ante mortem dispositions"@en-AU ;
    skos:narrower F2021L00308:240 ;
    skos:prefLabel "Item I244"@en-AU ;
    dcat:accessURL <https://www.legislation.gov.au/F2021L00308/2023-08-04/2023-08-04/text/original/epub/OEBPS/document_1/document_1.html#_Toc143604953> ;
    dcat:landingPage "https://www.legislation.gov.au/F2021L00308/2023-08-04/2023-08-04/text/original/epub/OEBPS/document_1/document_1.html#_Toc143604953"^^xsd:anyURI ;
    dcat:theme legcons:Item .

F2021L00308:245 a legcons:Item,
        owl:Class,
        dcat:Resource ;
    rdfs:label "Item - I245 9 24  Inspections of carcases and carcase parts and applying post mortem dispositions"@en-AU ;
    dct:isPartOf F2021L00308:240 ;
    dct:isReferencedBy F2021L00308: ;
    rdfs:comment "9 24  Inspections of carcases and carcase parts and applying post mortem dispositions - Abrievated Graph Key: I245"@en-AU ;
    skos:definition "9 24  Inspections of carcases and carcase parts and applying post mortem dispositions"@en-AU ;
    skos:narrower F2021L00308:240 ;
    skos:prefLabel "Item I245"@en-AU ;
    dcat:accessURL <https://www.legislation.gov.au/F2021L00308/2023-08-04/2023-08-04/text/original/epub/OEBPS/document_1/document_1.html#_Toc143604954> ;
    dcat:landingPage "https://www.legislation.gov.au/F2021L00308/2023-08-04/2023-08-04/text/original/epub/OEBPS/document_1/document_1.html#_Toc143604954"^^xsd:anyURI ;
    dcat:theme legcons:Item .

F2021L00308:246 a legcons:Item,
        owl:Class,
        dcat:Resource ;
    rdfs:label "Item - I246 9 25  Post mortem dispositions and related actions for rabbit carcases or carcase partsdisease or abnormality"@en-AU ;
    dct:isPartOf F2021L00308:240 ;
    dct:isReferencedBy F2021L00308: ;
    rdfs:comment "9 25  Post mortem dispositions and related actions for rabbit carcases or carcase partsdisease or abnormality - Abrievated Graph Key: I246"@en-AU ;
    skos:definition "9 25  Post mortem dispositions and related actions for rabbit carcases or carcase partsdisease or abnormality"@en-AU ;
    skos:narrower F2021L00308:240 ;
    skos:prefLabel "Item I246"@en-AU ;
    dcat:accessURL <https://www.legislation.gov.au/F2021L00308/2023-08-04/2023-08-04/text/original/epub/OEBPS/document_1/document_1.html#_Toc143604955> ;
    dcat:landingPage "https://www.legislation.gov.au/F2021L00308/2023-08-04/2023-08-04/text/original/epub/OEBPS/document_1/document_1.html#_Toc143604955"^^xsd:anyURI ;
    dcat:theme legcons:Item .

F2021L00308:247 a legcons:Item,
        owl:Class,
        dcat:Resource ;
    rdfs:label "Item - I247 9 26  Post mortem dispositions and related actions for ratite carcases or carcase partsdisease or abnormality"@en-AU ;
    dct:isPartOf F2021L00308:240 ;
    dct:isReferencedBy F2021L00308: ;
    rdfs:comment "9 26  Post mortem dispositions and related actions for ratite carcases or carcase partsdisease or abnormality - Abrievated Graph Key: I247"@en-AU ;
    skos:definition "9 26  Post mortem dispositions and related actions for ratite carcases or carcase partsdisease or abnormality"@en-AU ;
    skos:narrower F2021L00308:240 ;
    skos:prefLabel "Item I247"@en-AU ;
    dcat:accessURL <https://www.legislation.gov.au/F2021L00308/2023-08-04/2023-08-04/text/original/epub/OEBPS/document_1/document_1.html#_Toc143604956> ;
    dcat:landingPage "https://www.legislation.gov.au/F2021L00308/2023-08-04/2023-08-04/text/original/epub/OEBPS/document_1/document_1.html#_Toc143604956"^^xsd:anyURI ;
    dcat:theme legcons:Item .

F2021L00308:248 a legcons:Item,
        owl:Class,
        dcat:Resource ;
    rdfs:label "Item - I248 9 27  Inspections of rabbit meat ratite meat rabbit meat products and ratite meat products and applying dispositions"@en-AU ;
    dct:isPartOf F2021L00308:240 ;
    dct:isReferencedBy F2021L00308: ;
    rdfs:comment "9 27  Inspections of rabbit meat ratite meat rabbit meat products and ratite meat products and applying dispositions - Abrievated Graph Key: I248"@en-AU ;
    skos:definition "9 27  Inspections of rabbit meat ratite meat rabbit meat products and ratite meat products and applying dispositions"@en-AU ;
    skos:narrower F2021L00308:240 ;
    skos:prefLabel "Item I248"@en-AU ;
    dcat:accessURL <https://www.legislation.gov.au/F2021L00308/2023-08-04/2023-08-04/text/original/epub/OEBPS/document_1/document_1.html#_Toc143604957> ;
    dcat:landingPage "https://www.legislation.gov.au/F2021L00308/2023-08-04/2023-08-04/text/original/epub/OEBPS/document_1/document_1.html#_Toc143604957"^^xsd:anyURI ;
    dcat:theme legcons:Item .

F2021L00308:249 a legcons:Item,
        owl:Class,
        dcat:Resource ;
    rdfs:label "Item - I249 9 28  Applying decisions or dispositions subject to conditions and variation"@en-AU ;
    dct:isPartOf F2021L00308:240 ;
    dct:isReferencedBy F2021L00308: ;
    rdfs:comment "9 28  Applying decisions or dispositions subject to conditions and variation - Abrievated Graph Key: I249"@en-AU ;
    skos:definition "9 28  Applying decisions or dispositions subject to conditions and variation"@en-AU ;
    skos:narrower F2021L00308:240 ;
    skos:prefLabel "Item I249"@en-AU ;
    dcat:accessURL <https://www.legislation.gov.au/F2021L00308/2023-08-04/2023-08-04/text/original/epub/OEBPS/document_1/document_1.html#_Toc143604958> ;
    dcat:landingPage "https://www.legislation.gov.au/F2021L00308/2023-08-04/2023-08-04/text/original/epub/OEBPS/document_1/document_1.html#_Toc143604958"^^xsd:anyURI ;
    dcat:theme legcons:Item .

F2021L00308:25 a legcons:Item,
        owl:Class,
        dcat:Resource ;
    rdfs:label "Item - I25 2 7  Conditions of exemptionmatters to which Secretary must have regard"@en-AU ;
    dct:isPartOf F2021L00308:22 ;
    dct:isReferencedBy F2021L00308: ;
    rdfs:comment "2 7  Conditions of exemptionmatters to which Secretary must have regard - Abrievated Graph Key: I25"@en-AU ;
    skos:definition "2 7  Conditions of exemptionmatters to which Secretary must have regard"@en-AU ;
    skos:narrower F2021L00308:22 ;
    skos:prefLabel "Item I25"@en-AU ;
    dcat:accessURL <https://www.legislation.gov.au/F2021L00308/2023-08-04/2023-08-04/text/original/epub/OEBPS/document_1/document_1.html#_Toc143604734> ;
    dcat:landingPage "https://www.legislation.gov.au/F2021L00308/2023-08-04/2023-08-04/text/original/epub/OEBPS/document_1/document_1.html#_Toc143604734"^^xsd:anyURI ;
    dcat:theme legcons:Item .

F2021L00308:250 a legcons:Item,
        owl:Class,
        dcat:Resource ;
    rdfs:label "Item - I250 9 29  Stopping chain of operations temporarily or controlling rate of operations"@en-AU ;
    dct:isPartOf F2021L00308:240 ;
    dct:isReferencedBy F2021L00308: ;
    rdfs:comment "9 29  Stopping chain of operations temporarily or controlling rate of operations - Abrievated Graph Key: I250"@en-AU ;
    skos:definition "9 29  Stopping chain of operations temporarily or controlling rate of operations"@en-AU ;
    skos:narrower F2021L00308:240 ;
    skos:prefLabel "Item I250"@en-AU ;
    dcat:accessURL <https://www.legislation.gov.au/F2021L00308/2023-08-04/2023-08-04/text/original/epub/OEBPS/document_1/document_1.html#_Toc143604959> ;
    dcat:landingPage "https://www.legislation.gov.au/F2021L00308/2023-08-04/2023-08-04/text/original/epub/OEBPS/document_1/document_1.html#_Toc143604959"^^xsd:anyURI ;
    dcat:theme legcons:Item .

F2021L00308:251 a legcons:Item,
        owl:Class,
        dcat:Resource ;
    rdfs:label "Item - I251 9 30  Functions to be performed by veterinary officer or authorised officer acting under supervision of veterinary officer"@en-AU ;
    dct:isPartOf F2021L00308:240 ;
    dct:isReferencedBy F2021L00308: ;
    rdfs:comment "9 30  Functions to be performed by veterinary officer or authorised officer acting under supervision of veterinary officer - Abrievated Graph Key: I251"@en-AU ;
    skos:definition "9 30  Functions to be performed by veterinary officer or authorised officer acting under supervision of veterinary officer"@en-AU ;
    skos:narrower F2021L00308:240 ;
    skos:prefLabel "Item I251"@en-AU ;
    dcat:accessURL <https://www.legislation.gov.au/F2021L00308/2023-08-04/2023-08-04/text/original/epub/OEBPS/document_1/document_1.html#_Toc143604960> ;
    dcat:landingPage "https://www.legislation.gov.au/F2021L00308/2023-08-04/2023-08-04/text/original/epub/OEBPS/document_1/document_1.html#_Toc143604960"^^xsd:anyURI ;
    dcat:theme legcons:Item .

F2021L00308:252 a legcons:Item,
        owl:Class,
        dcat:Resource ;
    rdfs:label "Item - I252 9 31  Inspecting establishments and securing areas facilities equipment or other things"@en-AU ;
    dct:isPartOf F2021L00308:240 ;
    dct:isReferencedBy F2021L00308: ;
    rdfs:comment "9 31  Inspecting establishments and securing areas facilities equipment or other things - Abrievated Graph Key: I252"@en-AU ;
    skos:definition "9 31  Inspecting establishments and securing areas facilities equipment or other things"@en-AU ;
    skos:narrower F2021L00308:240 ;
    skos:prefLabel "Item I252"@en-AU ;
    dcat:accessURL <https://www.legislation.gov.au/F2021L00308/2023-08-04/2023-08-04/text/original/epub/OEBPS/document_1/document_1.html#_Toc143604961> ;
    dcat:landingPage "https://www.legislation.gov.au/F2021L00308/2023-08-04/2023-08-04/text/original/epub/OEBPS/document_1/document_1.html#_Toc143604961"^^xsd:anyURI ;
    dcat:theme legcons:Item .

F2021L00308:253 a legcons:Item,
        owl:Class,
        dcat:Resource ;
    rdfs:label "Item - I253 9 32  Securing and identifying establishment or conveyance etc"@en-AU ;
    dct:isPartOf F2021L00308:240 ;
    dct:isReferencedBy F2021L00308: ;
    rdfs:comment "9 32  Securing and identifying establishment or conveyance etc - Abrievated Graph Key: I253"@en-AU ;
    skos:definition "9 32  Securing and identifying establishment or conveyance etc"@en-AU ;
    skos:narrower F2021L00308:240 ;
    skos:prefLabel "Item I253"@en-AU ;
    dcat:accessURL <https://www.legislation.gov.au/F2021L00308/2023-08-04/2023-08-04/text/original/epub/OEBPS/document_1/document_1.html#_Toc143604962> ;
    dcat:landingPage "https://www.legislation.gov.au/F2021L00308/2023-08-04/2023-08-04/text/original/epub/OEBPS/document_1/document_1.html#_Toc143604962"^^xsd:anyURI ;
    dcat:theme legcons:Item .

F2021L00308:254 a legcons:Item,
        owl:Class,
        dcat:Resource ;
    rdfs:label "Item - I254 9 33  Interference with identified establishment or conveyance etc"@en-AU ;
    dct:isPartOf F2021L00308:240 ;
    dct:isReferencedBy F2021L00308: ;
    rdfs:comment "9 33  Interference with identified establishment or conveyance etc - Abrievated Graph Key: I254"@en-AU ;
    skos:definition "9 33  Interference with identified establishment or conveyance etc"@en-AU ;
    skos:narrower F2021L00308:240 ;
    skos:prefLabel "Item I254"@en-AU ;
    dcat:accessURL <https://www.legislation.gov.au/F2021L00308/2023-08-04/2023-08-04/text/original/epub/OEBPS/document_1/document_1.html#_Toc143604963> ;
    dcat:landingPage "https://www.legislation.gov.au/F2021L00308/2023-08-04/2023-08-04/text/original/epub/OEBPS/document_1/document_1.html#_Toc143604963"^^xsd:anyURI ;
    dcat:theme legcons:Item .

F2021L00308:255 a legcons:Item,
        owl:Class,
        dcat:Resource ;
    rdfs:label "Item - I255 9 34  Powers where integrity of prescribed rabbit meat ratite meat rabbit meat products or ratite meat products may not be able to be ensured"@en-AU ;
    dct:isPartOf F2021L00308:240 ;
    dct:isReferencedBy F2021L00308: ;
    rdfs:comment "9 34  Powers where integrity of prescribed rabbit meat ratite meat rabbit meat products or ratite meat products may not be able to be ensured - Abrievated Graph Key: I255"@en-AU ;
    skos:definition "9 34  Powers where integrity of prescribed rabbit meat ratite meat rabbit meat products or ratite meat products may not be able to be ensured"@en-AU ;
    skos:narrower F2021L00308:240 ;
    skos:prefLabel "Item I255"@en-AU ;
    dcat:accessURL <https://www.legislation.gov.au/F2021L00308/2023-08-04/2023-08-04/text/original/epub/OEBPS/document_1/document_1.html#_Toc143604964> ;
    dcat:landingPage "https://www.legislation.gov.au/F2021L00308/2023-08-04/2023-08-04/text/original/epub/OEBPS/document_1/document_1.html#_Toc143604964"^^xsd:anyURI ;
    dcat:theme legcons:Item .

F2021L00308:256 a legcons:Item,
        owl:Class,
        dcat:Resource ;
    rdfs:label "Item - I256 9 35  Giving certificate of condemnation"@en-AU ;
    dct:isPartOf F2021L00308:240 ;
    dct:isReferencedBy F2021L00308: ;
    rdfs:comment "9 35  Giving certificate of condemnation - Abrievated Graph Key: I256"@en-AU ;
    skos:definition "9 35  Giving certificate of condemnation"@en-AU ;
    skos:narrower F2021L00308:240 ;
    skos:prefLabel "Item I256"@en-AU ;
    dcat:accessURL <https://www.legislation.gov.au/F2021L00308/2023-08-04/2023-08-04/text/original/epub/OEBPS/document_1/document_1.html#_Toc143604965> ;
    dcat:landingPage "https://www.legislation.gov.au/F2021L00308/2023-08-04/2023-08-04/text/original/epub/OEBPS/document_1/document_1.html#_Toc143604965"^^xsd:anyURI ;
    dcat:theme legcons:Item .

F2021L00308:258 a legcons:Item,
        owl:Class,
        dcat:Resource ;
    rdfs:label "Item - I258 9 36  Other grounds for giving direction"@en-AU ;
    dct:isPartOf F2021L00308:257 ;
    dct:isReferencedBy F2021L00308: ;
    rdfs:comment "9 36  Other grounds for giving direction - Abrievated Graph Key: I258"@en-AU ;
    skos:definition "9 36  Other grounds for giving direction"@en-AU ;
    skos:narrower F2021L00308:257 ;
    skos:prefLabel "Item I258"@en-AU ;
    dcat:accessURL <https://www.legislation.gov.au/F2021L00308/2023-08-04/2023-08-04/text/original/epub/OEBPS/document_1/document_1.html#_Toc143604967> ;
    dcat:landingPage "https://www.legislation.gov.au/F2021L00308/2023-08-04/2023-08-04/text/original/epub/OEBPS/document_1/document_1.html#_Toc143604967"^^xsd:anyURI ;
    dcat:theme legcons:Item .

F2021L00308:26 a legcons:Item,
        owl:Class,
        dcat:Resource ;
    rdfs:label "Item - I26 2 8  Period of effect of exemption"@en-AU ;
    dct:isPartOf F2021L00308:22 ;
    dct:isReferencedBy F2021L00308: ;
    rdfs:comment "2 8  Period of effect of exemption - Abrievated Graph Key: I26"@en-AU ;
    skos:definition "2 8  Period of effect of exemption"@en-AU ;
    skos:narrower F2021L00308:22 ;
    skos:prefLabel "Item I26"@en-AU ;
    dcat:accessURL <https://www.legislation.gov.au/F2021L00308/2023-08-04/2023-08-04/text/original/epub/OEBPS/document_1/document_1.html#_Toc143604735> ;
    dcat:landingPage "https://www.legislation.gov.au/F2021L00308/2023-08-04/2023-08-04/text/original/epub/OEBPS/document_1/document_1.html#_Toc143604735"^^xsd:anyURI ;
    dcat:theme legcons:Item .

F2021L00308:260 a legcons:Item,
        owl:Class,
        dcat:Resource ;
    rdfs:label "Item - I260 9 37  Circumstances in which identity card need not be carried"@en-AU ;
    dct:isPartOf F2021L00308:259 ;
    dct:isReferencedBy F2021L00308: ;
    rdfs:comment "9 37  Circumstances in which identity card need not be carried - Abrievated Graph Key: I260"@en-AU ;
    skos:definition "9 37  Circumstances in which identity card need not be carried"@en-AU ;
    skos:narrower F2021L00308:259 ;
    skos:prefLabel "Item I260"@en-AU ;
    dcat:accessURL <https://www.legislation.gov.au/F2021L00308/2023-08-04/2023-08-04/text/original/epub/OEBPS/document_1/document_1.html#_Toc143604969> ;
    dcat:landingPage "https://www.legislation.gov.au/F2021L00308/2023-08-04/2023-08-04/text/original/epub/OEBPS/document_1/document_1.html#_Toc143604969"^^xsd:anyURI ;
    dcat:theme legcons:Item .

F2021L00308:262 a legcons:Item,
        owl:Class,
        dcat:Resource ;
    rdfs:label "Item - I262 10 1  Samples taken in exercising monitoring or investigation powers"@en-AU ;
    dct:isPartOf F2021L00308:261 ;
    dct:isReferencedBy F2021L00308: ;
    rdfs:comment "10 1  Samples taken in exercising monitoring or investigation powers - Abrievated Graph Key: I262"@en-AU ;
    skos:definition "10 1  Samples taken in exercising monitoring or investigation powers"@en-AU ;
    skos:narrower F2021L00308:261 ;
    skos:prefLabel "Item I262"@en-AU ;
    dcat:accessURL <https://www.legislation.gov.au/F2021L00308/2023-08-04/2023-08-04/text/original/epub/OEBPS/document_1/document_1.html#_Toc143604971> ;
    dcat:landingPage "https://www.legislation.gov.au/F2021L00308/2023-08-04/2023-08-04/text/original/epub/OEBPS/document_1/document_1.html#_Toc143604971"^^xsd:anyURI ;
    dcat:theme legcons:Item .

F2021L00308:263 a legcons:Item,
        owl:Class,
        dcat:Resource ;
    rdfs:label "Item - I263 10 2  Dealing with things seized in exercising investigation powers"@en-AU ;
    dct:isPartOf F2021L00308:261 ;
    dct:isReferencedBy F2021L00308: ;
    rdfs:comment "10 2  Dealing with things seized in exercising investigation powers - Abrievated Graph Key: I263"@en-AU ;
    skos:definition "10 2  Dealing with things seized in exercising investigation powers"@en-AU ;
    skos:narrower F2021L00308:261 ;
    skos:prefLabel "Item I263"@en-AU ;
    dcat:accessURL <https://www.legislation.gov.au/F2021L00308/2023-08-04/2023-08-04/text/original/epub/OEBPS/document_1/document_1.html#_Toc143604972> ;
    dcat:landingPage "https://www.legislation.gov.au/F2021L00308/2023-08-04/2023-08-04/text/original/epub/OEBPS/document_1/document_1.html#_Toc143604972"^^xsd:anyURI ;
    dcat:theme legcons:Item .

F2021L00308:266 a legcons:Item,
        owl:Class,
        dcat:Resource ;
    rdfs:label "Item - I266 11 1  Reviewable decisions"@en-AU ;
    dct:isPartOf F2021L00308:265 ;
    dct:isReferencedBy F2021L00308: ;
    rdfs:comment "11 1  Reviewable decisions - Abrievated Graph Key: I266"@en-AU ;
    skos:definition "11 1  Reviewable decisions"@en-AU ;
    skos:narrower F2021L00308:265 ;
    skos:prefLabel "Item I266"@en-AU ;
    dcat:accessURL <https://www.legislation.gov.au/F2021L00308/2023-08-04/2023-08-04/text/original/epub/OEBPS/document_1/document_1.html#_Toc143604975> ;
    dcat:landingPage "https://www.legislation.gov.au/F2021L00308/2023-08-04/2023-08-04/text/original/epub/OEBPS/document_1/document_1.html#_Toc143604975"^^xsd:anyURI ;
    dcat:theme legcons:Item .

F2021L00308:268 a legcons:Item,
        owl:Class,
        dcat:Resource ;
    rdfs:label "Item - I268 11 2  Purpose of this Part"@en-AU ;
    dct:isPartOf F2021L00308:267 ;
    dct:isReferencedBy F2021L00308: ;
    rdfs:comment "11 2  Purpose of this Part - Abrievated Graph Key: I268"@en-AU ;
    skos:definition "11 2  Purpose of this Part"@en-AU ;
    skos:narrower F2021L00308:267 ;
    skos:prefLabel "Item I268"@en-AU ;
    dcat:accessURL <https://www.legislation.gov.au/F2021L00308/2023-08-04/2023-08-04/text/original/epub/OEBPS/document_1/document_1.html#_Toc143604977> ;
    dcat:landingPage "https://www.legislation.gov.au/F2021L00308/2023-08-04/2023-08-04/text/original/epub/OEBPS/document_1/document_1.html#_Toc143604977"^^xsd:anyURI ;
    dcat:theme legcons:Item .

F2021L00308:269 a legcons:Item,
        owl:Class,
        dcat:Resource ;
    rdfs:label "Item - I269 11 3  General requirements for records"@en-AU ;
    dct:isPartOf F2021L00308:267 ;
    dct:isReferencedBy F2021L00308: ;
    rdfs:comment "11 3  General requirements for records - Abrievated Graph Key: I269"@en-AU ;
    skos:definition "11 3  General requirements for records"@en-AU ;
    skos:narrower F2021L00308:267 ;
    skos:prefLabel "Item I269"@en-AU ;
    dcat:accessURL <https://www.legislation.gov.au/F2021L00308/2023-08-04/2023-08-04/text/original/epub/OEBPS/document_1/document_1.html#_Toc143604978> ;
    dcat:landingPage "https://www.legislation.gov.au/F2021L00308/2023-08-04/2023-08-04/text/original/epub/OEBPS/document_1/document_1.html#_Toc143604978"^^xsd:anyURI ;
    dcat:theme legcons:Item .

F2021L00308:27 a legcons:Item,
        owl:Class,
        dcat:Resource ;
    rdfs:label "Item - I27 2 9  Variation of conditions of exemptionmatters to which Secretary must have regard"@en-AU ;
    dct:isPartOf F2021L00308:22 ;
    dct:isReferencedBy F2021L00308: ;
    rdfs:comment "2 9  Variation of conditions of exemptionmatters to which Secretary must have regard - Abrievated Graph Key: I27"@en-AU ;
    skos:definition "2 9  Variation of conditions of exemptionmatters to which Secretary must have regard"@en-AU ;
    skos:narrower F2021L00308:22 ;
    skos:prefLabel "Item I27"@en-AU ;
    dcat:accessURL <https://www.legislation.gov.au/F2021L00308/2023-08-04/2023-08-04/text/original/epub/OEBPS/document_1/document_1.html#_Toc143604736> ;
    dcat:landingPage "https://www.legislation.gov.au/F2021L00308/2023-08-04/2023-08-04/text/original/epub/OEBPS/document_1/document_1.html#_Toc143604736"^^xsd:anyURI ;
    dcat:theme legcons:Item .

F2021L00308:270 a legcons:Item,
        owl:Class,
        dcat:Resource ;
    rdfs:label "Item - I270 11 4  Government certificates"@en-AU ;
    dct:isPartOf F2021L00308:267 ;
    dct:isReferencedBy F2021L00308: ;
    rdfs:comment "11 4  Government certificates - Abrievated Graph Key: I270"@en-AU ;
    skos:definition "11 4  Government certificates"@en-AU ;
    skos:narrower F2021L00308:267 ;
    skos:prefLabel "Item I270"@en-AU ;
    dcat:accessURL <https://www.legislation.gov.au/F2021L00308/2023-08-04/2023-08-04/text/original/epub/OEBPS/document_1/document_1.html#_Toc143604979> ;
    dcat:landingPage "https://www.legislation.gov.au/F2021L00308/2023-08-04/2023-08-04/text/original/epub/OEBPS/document_1/document_1.html#_Toc143604979"^^xsd:anyURI ;
    dcat:theme legcons:Item .

F2021L00308:271 a legcons:Item,
        owl:Class,
        dcat:Resource ;
    rdfs:label "Item - I271 11 5  Export permits"@en-AU ;
    dct:isPartOf F2021L00308:267 ;
    dct:isReferencedBy F2021L00308: ;
    rdfs:comment "11 5  Export permits - Abrievated Graph Key: I271"@en-AU ;
    skos:definition "11 5  Export permits"@en-AU ;
    skos:narrower F2021L00308:267 ;
    skos:prefLabel "Item I271"@en-AU ;
    dcat:accessURL <https://www.legislation.gov.au/F2021L00308/2023-08-04/2023-08-04/text/original/epub/OEBPS/document_1/document_1.html#_Toc143604980> ;
    dcat:landingPage "https://www.legislation.gov.au/F2021L00308/2023-08-04/2023-08-04/text/original/epub/OEBPS/document_1/document_1.html#_Toc143604980"^^xsd:anyURI ;
    dcat:theme legcons:Item .

F2021L00308:272 a legcons:Item,
        owl:Class,
        dcat:Resource ;
    rdfs:label "Item - I272 11 6  Records to be retained by exporter"@en-AU ;
    dct:isPartOf F2021L00308:267 ;
    dct:isReferencedBy F2021L00308: ;
    rdfs:comment "11 6  Records to be retained by exporter - Abrievated Graph Key: I272"@en-AU ;
    skos:definition "11 6  Records to be retained by exporter"@en-AU ;
    skos:narrower F2021L00308:267 ;
    skos:prefLabel "Item I272"@en-AU ;
    dcat:accessURL <https://www.legislation.gov.au/F2021L00308/2023-08-04/2023-08-04/text/original/epub/OEBPS/document_1/document_1.html#_Toc143604981> ;
    dcat:landingPage "https://www.legislation.gov.au/F2021L00308/2023-08-04/2023-08-04/text/original/epub/OEBPS/document_1/document_1.html#_Toc143604981"^^xsd:anyURI ;
    dcat:theme legcons:Item .

F2021L00308:273 a legcons:Item,
        owl:Class,
        dcat:Resource ;
    rdfs:label "Item - I273 11 7  Records to be retained by occupier of registered establishment"@en-AU ;
    dct:isPartOf F2021L00308:267 ;
    dct:isReferencedBy F2021L00308: ;
    rdfs:comment "11 7  Records to be retained by occupier of registered establishment - Abrievated Graph Key: I273"@en-AU ;
    skos:definition "11 7  Records to be retained by occupier of registered establishment"@en-AU ;
    skos:narrower F2021L00308:267 ;
    skos:prefLabel "Item I273"@en-AU ;
    dcat:accessURL <https://www.legislation.gov.au/F2021L00308/2023-08-04/2023-08-04/text/original/epub/OEBPS/document_1/document_1.html#_Toc143604982> ;
    dcat:landingPage "https://www.legislation.gov.au/F2021L00308/2023-08-04/2023-08-04/text/original/epub/OEBPS/document_1/document_1.html#_Toc143604982"^^xsd:anyURI ;
    dcat:theme legcons:Item .

F2021L00308:274 a legcons:Item,
        owl:Class,
        dcat:Resource ;
    rdfs:label "Item - I274 11 8  Records to be retained by holder of approved arrangement"@en-AU ;
    dct:isPartOf F2021L00308:267 ;
    dct:isReferencedBy F2021L00308: ;
    rdfs:comment "11 8  Records to be retained by holder of approved arrangement - Abrievated Graph Key: I274"@en-AU ;
    skos:definition "11 8  Records to be retained by holder of approved arrangement"@en-AU ;
    skos:narrower F2021L00308:267 ;
    skos:prefLabel "Item I274"@en-AU ;
    dcat:accessURL <https://www.legislation.gov.au/F2021L00308/2023-08-04/2023-08-04/text/original/epub/OEBPS/document_1/document_1.html#_Toc143604983> ;
    dcat:landingPage "https://www.legislation.gov.au/F2021L00308/2023-08-04/2023-08-04/text/original/epub/OEBPS/document_1/document_1.html#_Toc143604983"^^xsd:anyURI ;
    dcat:theme legcons:Item .

F2021L00308:275 a legcons:Item,
        owl:Class,
        dcat:Resource ;
    rdfs:label "Item - I275 11 9  Records relating to official marks"@en-AU ;
    dct:isPartOf F2021L00308:267 ;
    dct:isReferencedBy F2021L00308: ;
    rdfs:comment "11 9  Records relating to official marks - Abrievated Graph Key: I275"@en-AU ;
    skos:definition "11 9  Records relating to official marks"@en-AU ;
    skos:narrower F2021L00308:267 ;
    skos:prefLabel "Item I275"@en-AU ;
    dcat:accessURL <https://www.legislation.gov.au/F2021L00308/2023-08-04/2023-08-04/text/original/epub/OEBPS/document_1/document_1.html#_Toc143604984> ;
    dcat:landingPage "https://www.legislation.gov.au/F2021L00308/2023-08-04/2023-08-04/text/original/epub/OEBPS/document_1/document_1.html#_Toc143604984"^^xsd:anyURI ;
    dcat:theme legcons:Item .

F2021L00308:276 a legcons:Item,
        owl:Class,
        dcat:Resource ;
    rdfs:label "Item - I276 11 10  Records relating to official marking devices"@en-AU ;
    dct:isPartOf F2021L00308:267 ;
    dct:isReferencedBy F2021L00308: ;
    rdfs:comment "11 10  Records relating to official marking devices - Abrievated Graph Key: I276"@en-AU ;
    skos:definition "11 10  Records relating to official marking devices"@en-AU ;
    skos:narrower F2021L00308:267 ;
    skos:prefLabel "Item I276"@en-AU ;
    dcat:accessURL <https://www.legislation.gov.au/F2021L00308/2023-08-04/2023-08-04/text/original/epub/OEBPS/document_1/document_1.html#_Toc143604985> ;
    dcat:landingPage "https://www.legislation.gov.au/F2021L00308/2023-08-04/2023-08-04/text/original/epub/OEBPS/document_1/document_1.html#_Toc143604985"^^xsd:anyURI ;
    dcat:theme legcons:Item .

F2021L00308:277 a legcons:Item,
        owl:Class,
        dcat:Resource ;
    rdfs:label "Item - I277 11 11  Records must not be altered or defaced during retention period"@en-AU ;
    dct:isPartOf F2021L00308:267 ;
    dct:isReferencedBy F2021L00308: ;
    rdfs:comment "11 11  Records must not be altered or defaced during retention period - Abrievated Graph Key: I277"@en-AU ;
    skos:definition "11 11  Records must not be altered or defaced during retention period"@en-AU ;
    skos:narrower F2021L00308:267 ;
    skos:prefLabel "Item I277"@en-AU ;
    dcat:accessURL <https://www.legislation.gov.au/F2021L00308/2023-08-04/2023-08-04/text/original/epub/OEBPS/document_1/document_1.html#_Toc143604986> ;
    dcat:landingPage "https://www.legislation.gov.au/F2021L00308/2023-08-04/2023-08-04/text/original/epub/OEBPS/document_1/document_1.html#_Toc143604986"^^xsd:anyURI ;
    dcat:theme legcons:Item .

F2021L00308:279 a legcons:Item,
        owl:Class,
        dcat:Resource ;
    rdfs:label "Item - I279 11 12  Storage of samples"@en-AU ;
    dct:isPartOf F2021L00308:278 ;
    dct:isReferencedBy F2021L00308: ;
    rdfs:comment "11 12  Storage of samples - Abrievated Graph Key: I279"@en-AU ;
    skos:definition "11 12  Storage of samples"@en-AU ;
    skos:narrower F2021L00308:278 ;
    skos:prefLabel "Item I279"@en-AU ;
    dcat:accessURL <https://www.legislation.gov.au/F2021L00308/2023-08-04/2023-08-04/text/original/epub/OEBPS/document_1/document_1.html#_Toc143604988> ;
    dcat:landingPage "https://www.legislation.gov.au/F2021L00308/2023-08-04/2023-08-04/text/original/epub/OEBPS/document_1/document_1.html#_Toc143604988"^^xsd:anyURI ;
    dcat:theme legcons:Item .

F2021L00308:28 a legcons:Item,
        owl:Class,
        dcat:Resource ;
    rdfs:label "Item - I28 2 10  Revocation of exemptionmatters to which Secretary must have regard"@en-AU ;
    dct:isPartOf F2021L00308:22 ;
    dct:isReferencedBy F2021L00308: ;
    rdfs:comment "2 10  Revocation of exemptionmatters to which Secretary must have regard - Abrievated Graph Key: I28"@en-AU ;
    skos:definition "2 10  Revocation of exemptionmatters to which Secretary must have regard"@en-AU ;
    skos:narrower F2021L00308:22 ;
    skos:prefLabel "Item I28"@en-AU ;
    dcat:accessURL <https://www.legislation.gov.au/F2021L00308/2023-08-04/2023-08-04/text/original/epub/OEBPS/document_1/document_1.html#_Toc143604737> ;
    dcat:landingPage "https://www.legislation.gov.au/F2021L00308/2023-08-04/2023-08-04/text/original/epub/OEBPS/document_1/document_1.html#_Toc143604737"^^xsd:anyURI ;
    dcat:theme legcons:Item .

F2021L00308:281 a legcons:Item,
        owl:Class,
        dcat:Resource ;
    rdfs:label "Item - I281 11 13  Division of compensation between owners"@en-AU ;
    dct:isPartOf F2021L00308:280 ;
    dct:isReferencedBy F2021L00308: ;
    rdfs:comment "11 13  Division of compensation between owners - Abrievated Graph Key: I281"@en-AU ;
    skos:definition "11 13  Division of compensation between owners"@en-AU ;
    skos:narrower F2021L00308:280 ;
    skos:prefLabel "Item I281"@en-AU ;
    dcat:accessURL <https://www.legislation.gov.au/F2021L00308/2023-08-04/2023-08-04/text/original/epub/OEBPS/document_1/document_1.html#_Toc143604990> ;
    dcat:landingPage "https://www.legislation.gov.au/F2021L00308/2023-08-04/2023-08-04/text/original/epub/OEBPS/document_1/document_1.html#_Toc143604990"^^xsd:anyURI ;
    dcat:theme legcons:Item .

F2021L00308:282 a legcons:Item,
        owl:Class,
        dcat:Resource ;
    rdfs:label "Item - I282 11 14  Amount of compensation"@en-AU ;
    dct:isPartOf F2021L00308:280 ;
    dct:isReferencedBy F2021L00308: ;
    rdfs:comment "11 14  Amount of compensation - Abrievated Graph Key: I282"@en-AU ;
    skos:definition "11 14  Amount of compensation"@en-AU ;
    skos:narrower F2021L00308:280 ;
    skos:prefLabel "Item I282"@en-AU ;
    dcat:accessURL <https://www.legislation.gov.au/F2021L00308/2023-08-04/2023-08-04/text/original/epub/OEBPS/document_1/document_1.html#_Toc143604991> ;
    dcat:landingPage "https://www.legislation.gov.au/F2021L00308/2023-08-04/2023-08-04/text/original/epub/OEBPS/document_1/document_1.html#_Toc143604991"^^xsd:anyURI ;
    dcat:theme legcons:Item .

F2021L00308:284 a legcons:Item,
        owl:Class,
        dcat:Resource ;
    rdfs:label "Item - I284 11 15  Circumstances in which relevant Commonwealth liability of a person is taken to have been paid"@en-AU ;
    dct:isPartOf F2021L00308:283 ;
    dct:isReferencedBy F2021L00308: ;
    rdfs:comment "11 15  Circumstances in which relevant Commonwealth liability of a person is taken to have been paid - Abrievated Graph Key: I284"@en-AU ;
    skos:definition "11 15  Circumstances in which relevant Commonwealth liability of a person is taken to have been paid"@en-AU ;
    skos:narrower F2021L00308:283 ;
    skos:prefLabel "Item I284"@en-AU ;
    dcat:accessURL <https://www.legislation.gov.au/F2021L00308/2023-08-04/2023-08-04/text/original/epub/OEBPS/document_1/document_1.html#_Toc143604993> ;
    dcat:landingPage "https://www.legislation.gov.au/F2021L00308/2023-08-04/2023-08-04/text/original/epub/OEBPS/document_1/document_1.html#_Toc143604993"^^xsd:anyURI ;
    dcat:theme legcons:Item .

F2021L00308:287 a legcons:Item,
        owl:Class,
        dcat:Resource ;
    rdfs:label "Item - I287 12 1  Definitions"@en-AU ;
    dct:isPartOf F2021L00308:286 ;
    dct:isReferencedBy F2021L00308: ;
    rdfs:comment "12 1  Definitions - Abrievated Graph Key: I287"@en-AU ;
    skos:definition "12 1  Definitions"@en-AU ;
    skos:narrower F2021L00308:286 ;
    skos:prefLabel "Item I287"@en-AU ;
    dcat:accessURL <https://www.legislation.gov.au/F2021L00308/2023-08-04/2023-08-04/text/original/epub/OEBPS/document_1/document_1.html#_Toc143604996> ;
    dcat:landingPage "https://www.legislation.gov.au/F2021L00308/2023-08-04/2023-08-04/text/original/epub/OEBPS/document_1/document_1.html#_Toc143604996"^^xsd:anyURI ;
    dcat:theme legcons:Item .

F2021L00308:290 a legcons:Item,
        owl:Class,
        dcat:Resource ;
    rdfs:label "Item - I290 12 2  Person approved before commencement time to manufacture an official mark"@en-AU ;
    dct:isPartOf F2021L00308:289 ;
    dct:isReferencedBy F2021L00308: ;
    rdfs:comment "12 2  Person approved before commencement time to manufacture an official mark - Abrievated Graph Key: I290"@en-AU ;
    skos:definition "12 2  Person approved before commencement time to manufacture an official mark"@en-AU ;
    skos:narrower F2021L00308:289 ;
    skos:prefLabel "Item I290"@en-AU ;
    dcat:accessURL <https://www.legislation.gov.au/F2021L00308/2023-08-04/2023-08-04/text/original/epub/OEBPS/document_1/document_1.html#_Toc143604999> ;
    dcat:landingPage "https://www.legislation.gov.au/F2021L00308/2023-08-04/2023-08-04/text/original/epub/OEBPS/document_1/document_1.html#_Toc143604999"^^xsd:anyURI ;
    dcat:theme legcons:Item .

F2021L00308:291 a legcons:Item,
        owl:Class,
        dcat:Resource ;
    rdfs:label "Item - I291 12 3  Person approved before commencement time to possess an official mark"@en-AU ;
    dct:isPartOf F2021L00308:289 ;
    dct:isReferencedBy F2021L00308: ;
    rdfs:comment "12 3  Person approved before commencement time to possess an official mark - Abrievated Graph Key: I291"@en-AU ;
    skos:definition "12 3  Person approved before commencement time to possess an official mark"@en-AU ;
    skos:narrower F2021L00308:289 ;
    skos:prefLabel "Item I291"@en-AU ;
    dcat:accessURL <https://www.legislation.gov.au/F2021L00308/2023-08-04/2023-08-04/text/original/epub/OEBPS/document_1/document_1.html#_Toc143605000> ;
    dcat:landingPage "https://www.legislation.gov.au/F2021L00308/2023-08-04/2023-08-04/text/original/epub/OEBPS/document_1/document_1.html#_Toc143605000"^^xsd:anyURI ;
    dcat:theme legcons:Item .

F2021L00308:292 a legcons:Item,
        owl:Class,
        dcat:Resource ;
    rdfs:label "Item - I292 12 4  Person approved before commencement time to apply an official mark"@en-AU ;
    dct:isPartOf F2021L00308:289 ;
    dct:isReferencedBy F2021L00308: ;
    rdfs:comment "12 4  Person approved before commencement time to apply an official mark - Abrievated Graph Key: I292"@en-AU ;
    skos:definition "12 4  Person approved before commencement time to apply an official mark"@en-AU ;
    skos:narrower F2021L00308:289 ;
    skos:prefLabel "Item I292"@en-AU ;
    dcat:accessURL <https://www.legislation.gov.au/F2021L00308/2023-08-04/2023-08-04/text/original/epub/OEBPS/document_1/document_1.html#_Toc143605001> ;
    dcat:landingPage "https://www.legislation.gov.au/F2021L00308/2023-08-04/2023-08-04/text/original/epub/OEBPS/document_1/document_1.html#_Toc143605001"^^xsd:anyURI ;
    dcat:theme legcons:Item .

F2021L00308:294 a legcons:Item,
        owl:Class,
        dcat:Resource ;
    rdfs:label "Item - I294 12 5  Person approved before commencement time to manufacture an official marking device"@en-AU ;
    dct:isPartOf F2021L00308:293 ;
    dct:isReferencedBy F2021L00308: ;
    rdfs:comment "12 5  Person approved before commencement time to manufacture an official marking device - Abrievated Graph Key: I294"@en-AU ;
    skos:definition "12 5  Person approved before commencement time to manufacture an official marking device"@en-AU ;
    skos:narrower F2021L00308:293 ;
    skos:prefLabel "Item I294"@en-AU ;
    dcat:accessURL <https://www.legislation.gov.au/F2021L00308/2023-08-04/2023-08-04/text/original/epub/OEBPS/document_1/document_1.html#_Toc143605003> ;
    dcat:landingPage "https://www.legislation.gov.au/F2021L00308/2023-08-04/2023-08-04/text/original/epub/OEBPS/document_1/document_1.html#_Toc143605003"^^xsd:anyURI ;
    dcat:theme legcons:Item .

F2021L00308:295 a legcons:Item,
        owl:Class,
        dcat:Resource ;
    rdfs:label "Item - I295 12 6  Person approved before commencement time to possess an official marking device"@en-AU ;
    dct:isPartOf F2021L00308:293 ;
    dct:isReferencedBy F2021L00308: ;
    rdfs:comment "12 6  Person approved before commencement time to possess an official marking device - Abrievated Graph Key: I295"@en-AU ;
    skos:definition "12 6  Person approved before commencement time to possess an official marking device"@en-AU ;
    skos:narrower F2021L00308:293 ;
    skos:prefLabel "Item I295"@en-AU ;
    dcat:accessURL <https://www.legislation.gov.au/F2021L00308/2023-08-04/2023-08-04/text/original/epub/OEBPS/document_1/document_1.html#_Toc143605004> ;
    dcat:landingPage "https://www.legislation.gov.au/F2021L00308/2023-08-04/2023-08-04/text/original/epub/OEBPS/document_1/document_1.html#_Toc143605004"^^xsd:anyURI ;
    dcat:theme legcons:Item .

F2021L00308:297 a legcons:Item,
        owl:Class,
        dcat:Resource ;
    rdfs:label "Item - I297 12 7  Decision or disposition applied but not complied with before commencement time"@en-AU ;
    dct:isPartOf F2021L00308:296 ;
    dct:isReferencedBy F2021L00308: ;
    rdfs:comment "12 7  Decision or disposition applied but not complied with before commencement time - Abrievated Graph Key: I297"@en-AU ;
    skos:definition "12 7  Decision or disposition applied but not complied with before commencement time"@en-AU ;
    skos:narrower F2021L00308:296 ;
    skos:prefLabel "Item I297"@en-AU ;
    dcat:accessURL <https://www.legislation.gov.au/F2021L00308/2023-08-04/2023-08-04/text/original/epub/OEBPS/document_1/document_1.html#_Toc143605006> ;
    dcat:landingPage "https://www.legislation.gov.au/F2021L00308/2023-08-04/2023-08-04/text/original/epub/OEBPS/document_1/document_1.html#_Toc143605006"^^xsd:anyURI ;
    dcat:theme legcons:Item .

F2021L00308:3 a legcons:Item,
        owl:Class,
        dcat:Resource ;
    rdfs:label "Item - I3 1 1  Name"@en-AU ;
    dct:isPartOf F2021L00308:1 ;
    dct:isReferencedBy F2021L00308: ;
    rdfs:comment "1 1  Name - Abrievated Graph Key: I3"@en-AU ;
    skos:definition "1 1  Name"@en-AU ;
    skos:narrower F2021L00308:1 ;
    skos:prefLabel "Item I3"@en-AU ;
    dcat:accessURL <https://www.legislation.gov.au/F2021L00308/2023-08-04/2023-08-04/text/original/epub/OEBPS/document_1/document_1.html#_Toc143604712> ;
    dcat:landingPage "https://www.legislation.gov.au/F2021L00308/2023-08-04/2023-08-04/text/original/epub/OEBPS/document_1/document_1.html#_Toc143604712"^^xsd:anyURI ;
    dcat:theme legcons:Item .

F2021L00308:30 a legcons:Item,
        owl:Class,
        dcat:Resource ;
    rdfs:label "Item - I30 2 11  When government certificate may be issued in relation to rabbit meat ratite meat rabbit meat products or ratite meat products"@en-AU ;
    dct:isPartOf F2021L00308:29 ;
    dct:isReferencedBy F2021L00308: ;
    rdfs:comment "2 11  When government certificate may be issued in relation to rabbit meat ratite meat rabbit meat products or ratite meat products - Abrievated Graph Key: I30"@en-AU ;
    skos:definition "2 11  When government certificate may be issued in relation to rabbit meat ratite meat rabbit meat products or ratite meat products"@en-AU ;
    skos:narrower F2021L00308:29 ;
    skos:prefLabel "Item I30"@en-AU ;
    dcat:accessURL <https://www.legislation.gov.au/F2021L00308/2023-08-04/2023-08-04/text/original/epub/OEBPS/document_1/document_1.html#_Toc143604739> ;
    dcat:landingPage "https://www.legislation.gov.au/F2021L00308/2023-08-04/2023-08-04/text/original/epub/OEBPS/document_1/document_1.html#_Toc143604739"^^xsd:anyURI ;
    dcat:theme legcons:Item .

F2021L00308:300 a legcons:Item,
        owl:Class,
        dcat:Resource ;
    rdfs:label "Item - I300 1  Post mortem dispositions and related actions for rabbit carcases or carcase partsdisease or abnormality"@en-AU ;
    dct:isPartOf F2021L00308:299 ;
    dct:isReferencedBy F2021L00308: ;
    rdfs:comment "1  Post mortem dispositions and related actions for rabbit carcases or carcase partsdisease or abnormality - Abrievated Graph Key: I300"@en-AU ;
    skos:definition "1  Post mortem dispositions and related actions for rabbit carcases or carcase partsdisease or abnormality"@en-AU ;
    skos:narrower F2021L00308:299 ;
    skos:prefLabel "Item I300"@en-AU ;
    dcat:accessURL <https://www.legislation.gov.au/F2021L00308/2023-08-04/2023-08-04/text/original/epub/OEBPS/document_1/document_1.html#_Toc143605009> ;
    dcat:landingPage "https://www.legislation.gov.au/F2021L00308/2023-08-04/2023-08-04/text/original/epub/OEBPS/document_1/document_1.html#_Toc143605009"^^xsd:anyURI ;
    dcat:theme legcons:Item .

F2021L00308:302 a legcons:Item,
        owl:Class,
        dcat:Resource ;
    rdfs:label "Item - I302 2  Post mortem dispositions and related actions for ratite carcases or carcase partsdisease or abnormality"@en-AU ;
    dct:isPartOf F2021L00308:301 ;
    dct:isReferencedBy F2021L00308: ;
    rdfs:comment "2  Post mortem dispositions and related actions for ratite carcases or carcase partsdisease or abnormality - Abrievated Graph Key: I302"@en-AU ;
    skos:definition "2  Post mortem dispositions and related actions for ratite carcases or carcase partsdisease or abnormality"@en-AU ;
    skos:narrower F2021L00308:301 ;
    skos:prefLabel "Item I302"@en-AU ;
    dcat:accessURL <https://www.legislation.gov.au/F2021L00308/2023-08-04/2023-08-04/text/original/epub/OEBPS/document_1/document_1.html#_Toc143605011> ;
    dcat:landingPage "https://www.legislation.gov.au/F2021L00308/2023-08-04/2023-08-04/text/original/epub/OEBPS/document_1/document_1.html#_Toc143605011"^^xsd:anyURI ;
    dcat:theme legcons:Item .

F2021L00308:304 a legcons:Item,
        owl:Class,
        dcat:Resource ;
    rdfs:label "Item - I304 Endnote 1 About the endnotes"@en-AU ;
    dct:isPartOf F2021L00308:303 ;
    dct:isReferencedBy F2021L00308: ;
    rdfs:comment "Endnote 1 About the endnotes - Abrievated Graph Key: I304"@en-AU ;
    skos:definition "Endnote 1 About the endnotes"@en-AU ;
    skos:narrower F2021L00308:303 ;
    skos:prefLabel "Item I304"@en-AU ;
    dcat:accessURL <https://www.legislation.gov.au/F2021L00308/2023-08-04/2023-08-04/text/original/epub/OEBPS/document_1/document_1.html#_Toc143605013> ;
    dcat:landingPage "https://www.legislation.gov.au/F2021L00308/2023-08-04/2023-08-04/text/original/epub/OEBPS/document_1/document_1.html#_Toc143605013"^^xsd:anyURI ;
    dcat:theme legcons:Item .

F2021L00308:305 a legcons:Item,
        owl:Class,
        dcat:Resource ;
    rdfs:label "Item - I305 Endnote 2 Abbreviation key"@en-AU ;
    dct:isPartOf F2021L00308:303 ;
    dct:isReferencedBy F2021L00308: ;
    rdfs:comment "Endnote 2 Abbreviation key - Abrievated Graph Key: I305"@en-AU ;
    skos:definition "Endnote 2 Abbreviation key"@en-AU ;
    skos:narrower F2021L00308:303 ;
    skos:prefLabel "Item I305"@en-AU ;
    dcat:accessURL <https://www.legislation.gov.au/F2021L00308/2023-08-04/2023-08-04/text/original/epub/OEBPS/document_1/document_1.html#_Toc143605014> ;
    dcat:landingPage "https://www.legislation.gov.au/F2021L00308/2023-08-04/2023-08-04/text/original/epub/OEBPS/document_1/document_1.html#_Toc143605014"^^xsd:anyURI ;
    dcat:theme legcons:Item .

F2021L00308:306 a legcons:Item,
        owl:Class,
        dcat:Resource ;
    rdfs:label "Item - I306 Endnote 3 Legislation history"@en-AU ;
    dct:isPartOf F2021L00308:303 ;
    dct:isReferencedBy F2021L00308: ;
    rdfs:comment "Endnote 3 Legislation history - Abrievated Graph Key: I306"@en-AU ;
    skos:definition "Endnote 3 Legislation history"@en-AU ;
    skos:narrower F2021L00308:303 ;
    skos:prefLabel "Item I306"@en-AU ;
    dcat:accessURL <https://www.legislation.gov.au/F2021L00308/2023-08-04/2023-08-04/text/original/epub/OEBPS/document_1/document_1.html#_Toc143605015> ;
    dcat:landingPage "https://www.legislation.gov.au/F2021L00308/2023-08-04/2023-08-04/text/original/epub/OEBPS/document_1/document_1.html#_Toc143605015"^^xsd:anyURI ;
    dcat:theme legcons:Item .

F2021L00308:307 a legcons:Item,
        owl:Class,
        dcat:Resource ;
    rdfs:label "Item - I307 Endnote 4 Amendment history"@en-AU ;
    dct:isPartOf F2021L00308:303 ;
    dct:isReferencedBy F2021L00308: ;
    rdfs:comment "Endnote 4 Amendment history - Abrievated Graph Key: I307"@en-AU ;
    skos:definition "Endnote 4 Amendment history"@en-AU ;
    skos:narrower F2021L00308:303 ;
    skos:prefLabel "Item I307"@en-AU ;
    dcat:accessURL <https://www.legislation.gov.au/F2021L00308/2023-08-04/2023-08-04/text/original/epub/OEBPS/document_1/document_1.html#_Toc143605016> ;
    dcat:landingPage "https://www.legislation.gov.au/F2021L00308/2023-08-04/2023-08-04/text/original/epub/OEBPS/document_1/document_1.html#_Toc143605016"^^xsd:anyURI ;
    dcat:theme legcons:Item .

F2021L00308:31 a legcons:Item,
        owl:Class,
        dcat:Resource ;
    rdfs:label "Item - I31 2 12  Declaration to accompany application for government certificate"@en-AU ;
    dct:isPartOf F2021L00308:29 ;
    dct:isReferencedBy F2021L00308: ;
    rdfs:comment "2 12  Declaration to accompany application for government certificate - Abrievated Graph Key: I31"@en-AU ;
    skos:definition "2 12  Declaration to accompany application for government certificate"@en-AU ;
    skos:narrower F2021L00308:29 ;
    skos:prefLabel "Item I31"@en-AU ;
    dcat:accessURL <https://www.legislation.gov.au/F2021L00308/2023-08-04/2023-08-04/text/original/epub/OEBPS/document_1/document_1.html#_Toc143604740> ;
    dcat:landingPage "https://www.legislation.gov.au/F2021L00308/2023-08-04/2023-08-04/text/original/epub/OEBPS/document_1/document_1.html#_Toc143604740"^^xsd:anyURI ;
    dcat:theme legcons:Item .

F2021L00308:32 a legcons:Item,
        owl:Class,
        dcat:Resource ;
    rdfs:label "Item - I32 2 13  Circumstances for refusing to issue government certificate"@en-AU ;
    dct:isPartOf F2021L00308:29 ;
    dct:isReferencedBy F2021L00308: ;
    rdfs:comment "2 13  Circumstances for refusing to issue government certificate - Abrievated Graph Key: I32"@en-AU ;
    skos:definition "2 13  Circumstances for refusing to issue government certificate"@en-AU ;
    skos:narrower F2021L00308:29 ;
    skos:prefLabel "Item I32"@en-AU ;
    dcat:accessURL <https://www.legislation.gov.au/F2021L00308/2023-08-04/2023-08-04/text/original/epub/OEBPS/document_1/document_1.html#_Toc143604741> ;
    dcat:landingPage "https://www.legislation.gov.au/F2021L00308/2023-08-04/2023-08-04/text/original/epub/OEBPS/document_1/document_1.html#_Toc143604741"^^xsd:anyURI ;
    dcat:theme legcons:Item .

F2021L00308:33 a legcons:Item,
        owl:Class,
        dcat:Resource ;
    rdfs:label "Item - I33 2 14  Changes that require holder of certificate to give additional or corrected information to the issuing body"@en-AU ;
    dct:isPartOf F2021L00308:29 ;
    dct:isReferencedBy F2021L00308: ;
    rdfs:comment "2 14  Changes that require holder of certificate to give additional or corrected information to the issuing body - Abrievated Graph Key: I33"@en-AU ;
    skos:definition "2 14  Changes that require holder of certificate to give additional or corrected information to the issuing body"@en-AU ;
    skos:narrower F2021L00308:29 ;
    skos:prefLabel "Item I33"@en-AU ;
    dcat:accessURL <https://www.legislation.gov.au/F2021L00308/2023-08-04/2023-08-04/text/original/epub/OEBPS/document_1/document_1.html#_Toc143604742> ;
    dcat:landingPage "https://www.legislation.gov.au/F2021L00308/2023-08-04/2023-08-04/text/original/epub/OEBPS/document_1/document_1.html#_Toc143604742"^^xsd:anyURI ;
    dcat:theme legcons:Item .

F2021L00308:34 a legcons:Item,
        owl:Class,
        dcat:Resource ;
    rdfs:label "Item - I34 2 15  Return of government certificate"@en-AU ;
    dct:isPartOf F2021L00308:29 ;
    dct:isReferencedBy F2021L00308: ;
    rdfs:comment "2 15  Return of government certificate - Abrievated Graph Key: I34"@en-AU ;
    skos:definition "2 15  Return of government certificate"@en-AU ;
    skos:narrower F2021L00308:29 ;
    skos:prefLabel "Item I34"@en-AU ;
    dcat:accessURL <https://www.legislation.gov.au/F2021L00308/2023-08-04/2023-08-04/text/original/epub/OEBPS/document_1/document_1.html#_Toc143604743> ;
    dcat:landingPage "https://www.legislation.gov.au/F2021L00308/2023-08-04/2023-08-04/text/original/epub/OEBPS/document_1/document_1.html#_Toc143604743"^^xsd:anyURI ;
    dcat:theme legcons:Item .

F2021L00308:37 a legcons:Item,
        owl:Class,
        dcat:Resource ;
    rdfs:label "Item - I37 4 1  Purpose of this Part"@en-AU ;
    dct:isPartOf F2021L00308:36 ;
    dct:isReferencedBy F2021L00308: ;
    rdfs:comment "4 1  Purpose of this Part - Abrievated Graph Key: I37"@en-AU ;
    skos:definition "4 1  Purpose of this Part"@en-AU ;
    skos:narrower F2021L00308:36 ;
    skos:prefLabel "Item I37"@en-AU ;
    dcat:accessURL <https://www.legislation.gov.au/F2021L00308/2023-08-04/2023-08-04/text/original/epub/OEBPS/document_1/document_1.html#_Toc143604746> ;
    dcat:landingPage "https://www.legislation.gov.au/F2021L00308/2023-08-04/2023-08-04/text/original/epub/OEBPS/document_1/document_1.html#_Toc143604746"^^xsd:anyURI ;
    dcat:theme legcons:Item .

F2021L00308:38 a legcons:Item,
        owl:Class,
        dcat:Resource ;
    rdfs:label "Item - I38 4 2  Operations must be carried out in a way that will ensure requirements of the Act are complied with"@en-AU ;
    dct:isPartOf F2021L00308:36 ;
    dct:isReferencedBy F2021L00308: ;
    rdfs:comment "4 2  Operations must be carried out in a way that will ensure requirements of the Act are complied with - Abrievated Graph Key: I38"@en-AU ;
    skos:definition "4 2  Operations must be carried out in a way that will ensure requirements of the Act are complied with"@en-AU ;
    skos:narrower F2021L00308:36 ;
    skos:prefLabel "Item I38"@en-AU ;
    dcat:accessURL <https://www.legislation.gov.au/F2021L00308/2023-08-04/2023-08-04/text/original/epub/OEBPS/document_1/document_1.html#_Toc143604747> ;
    dcat:landingPage "https://www.legislation.gov.au/F2021L00308/2023-08-04/2023-08-04/text/original/epub/OEBPS/document_1/document_1.html#_Toc143604747"^^xsd:anyURI ;
    dcat:theme legcons:Item .

F2021L00308:39 a legcons:Item,
        owl:Class,
        dcat:Resource ;
    rdfs:label "Item - I39 4 3  Requirements of Australian Meat Standard must be met"@en-AU ;
    dct:isPartOf F2021L00308:36 ;
    dct:isReferencedBy F2021L00308: ;
    rdfs:comment "4 3  Requirements of Australian Meat Standard must be met - Abrievated Graph Key: I39"@en-AU ;
    skos:definition "4 3  Requirements of Australian Meat Standard must be met"@en-AU ;
    skos:narrower F2021L00308:36 ;
    skos:prefLabel "Item I39"@en-AU ;
    dcat:accessURL <https://www.legislation.gov.au/F2021L00308/2023-08-04/2023-08-04/text/original/epub/OEBPS/document_1/document_1.html#_Toc143604748> ;
    dcat:landingPage "https://www.legislation.gov.au/F2021L00308/2023-08-04/2023-08-04/text/original/epub/OEBPS/document_1/document_1.html#_Toc143604748"^^xsd:anyURI ;
    dcat:theme legcons:Item .

F2021L00308:4 a legcons:Item,
        owl:Class,
        dcat:Resource ;
    rdfs:label "Item - I4 1 3  Authority"@en-AU ;
    dct:isPartOf F2021L00308:1 ;
    dct:isReferencedBy F2021L00308: ;
    rdfs:comment "1 3  Authority - Abrievated Graph Key: I4"@en-AU ;
    skos:definition "1 3  Authority"@en-AU ;
    skos:narrower F2021L00308:1 ;
    skos:prefLabel "Item I4"@en-AU ;
    dcat:accessURL <https://www.legislation.gov.au/F2021L00308/2023-08-04/2023-08-04/text/original/epub/OEBPS/document_1/document_1.html#_Toc143604713> ;
    dcat:landingPage "https://www.legislation.gov.au/F2021L00308/2023-08-04/2023-08-04/text/original/epub/OEBPS/document_1/document_1.html#_Toc143604713"^^xsd:anyURI ;
    dcat:theme legcons:Item .

F2021L00308:40 a legcons:Item,
        owl:Class,
        dcat:Resource ;
    rdfs:label "Item - I40 4 4  Equipment facilities and essential services"@en-AU ;
    dct:isPartOf F2021L00308:36 ;
    dct:isReferencedBy F2021L00308: ;
    rdfs:comment "4 4  Equipment facilities and essential services - Abrievated Graph Key: I40"@en-AU ;
    skos:definition "4 4  Equipment facilities and essential services"@en-AU ;
    skos:narrower F2021L00308:36 ;
    skos:prefLabel "Item I40"@en-AU ;
    dcat:accessURL <https://www.legislation.gov.au/F2021L00308/2023-08-04/2023-08-04/text/original/epub/OEBPS/document_1/document_1.html#_Toc143604749> ;
    dcat:landingPage "https://www.legislation.gov.au/F2021L00308/2023-08-04/2023-08-04/text/original/epub/OEBPS/document_1/document_1.html#_Toc143604749"^^xsd:anyURI ;
    dcat:theme legcons:Item .

F2021L00308:41 a legcons:Item,
        owl:Class,
        dcat:Resource ;
    rdfs:label "Item - I41 4 5  Areas where post mortem inspections are carried out"@en-AU ;
    dct:isPartOf F2021L00308:36 ;
    dct:isReferencedBy F2021L00308: ;
    rdfs:comment "4 5  Areas where post mortem inspections are carried out - Abrievated Graph Key: I41"@en-AU ;
    skos:definition "4 5  Areas where post mortem inspections are carried out"@en-AU ;
    skos:narrower F2021L00308:36 ;
    skos:prefLabel "Item I41"@en-AU ;
    dcat:accessURL <https://www.legislation.gov.au/F2021L00308/2023-08-04/2023-08-04/text/original/epub/OEBPS/document_1/document_1.html#_Toc143604750> ;
    dcat:landingPage "https://www.legislation.gov.au/F2021L00308/2023-08-04/2023-08-04/text/original/epub/OEBPS/document_1/document_1.html#_Toc143604750"^^xsd:anyURI ;
    dcat:theme legcons:Item .

F2021L00308:42 a legcons:Item,
        owl:Class,
        dcat:Resource ;
    rdfs:label "Item - I42 4 6  Meat examination facility"@en-AU ;
    dct:isPartOf F2021L00308:36 ;
    dct:isReferencedBy F2021L00308: ;
    rdfs:comment "4 6  Meat examination facility - Abrievated Graph Key: I42"@en-AU ;
    skos:definition "4 6  Meat examination facility"@en-AU ;
    skos:narrower F2021L00308:36 ;
    skos:prefLabel "Item I42"@en-AU ;
    dcat:accessURL <https://www.legislation.gov.au/F2021L00308/2023-08-04/2023-08-04/text/original/epub/OEBPS/document_1/document_1.html#_Toc143604751> ;
    dcat:landingPage "https://www.legislation.gov.au/F2021L00308/2023-08-04/2023-08-04/text/original/epub/OEBPS/document_1/document_1.html#_Toc143604751"^^xsd:anyURI ;
    dcat:theme legcons:Item .

F2021L00308:43 a legcons:Item,
        owl:Class,
        dcat:Resource ;
    rdfs:label "Item - I43 4 7  Slaughter establishments must have laboratory facility"@en-AU ;
    dct:isPartOf F2021L00308:36 ;
    dct:isReferencedBy F2021L00308: ;
    rdfs:comment "4 7  Slaughter establishments must have laboratory facility - Abrievated Graph Key: I43"@en-AU ;
    skos:definition "4 7  Slaughter establishments must have laboratory facility"@en-AU ;
    skos:narrower F2021L00308:36 ;
    skos:prefLabel "Item I43"@en-AU ;
    dcat:accessURL <https://www.legislation.gov.au/F2021L00308/2023-08-04/2023-08-04/text/original/epub/OEBPS/document_1/document_1.html#_Toc143604752> ;
    dcat:landingPage "https://www.legislation.gov.au/F2021L00308/2023-08-04/2023-08-04/text/original/epub/OEBPS/document_1/document_1.html#_Toc143604752"^^xsd:anyURI ;
    dcat:theme legcons:Item .

F2021L00308:44 a legcons:Item,
        owl:Class,
        dcat:Resource ;
    rdfs:label "Item - I44 4 8  Areas for preparation of prescribed rabbit meat or rabbit meat products"@en-AU ;
    dct:isPartOf F2021L00308:36 ;
    dct:isReferencedBy F2021L00308: ;
    rdfs:comment "4 8  Areas for preparation of prescribed rabbit meat or rabbit meat products - Abrievated Graph Key: I44"@en-AU ;
    skos:definition "4 8  Areas for preparation of prescribed rabbit meat or rabbit meat products"@en-AU ;
    skos:narrower F2021L00308:36 ;
    skos:prefLabel "Item I44"@en-AU ;
    dcat:accessURL <https://www.legislation.gov.au/F2021L00308/2023-08-04/2023-08-04/text/original/epub/OEBPS/document_1/document_1.html#_Toc143604753> ;
    dcat:landingPage "https://www.legislation.gov.au/F2021L00308/2023-08-04/2023-08-04/text/original/epub/OEBPS/document_1/document_1.html#_Toc143604753"^^xsd:anyURI ;
    dcat:theme legcons:Item .

F2021L00308:45 a legcons:Item,
        owl:Class,
        dcat:Resource ;
    rdfs:label "Item - I45 4 9  Areas for preparation of prescribed ratite meat or ratite meat products"@en-AU ;
    dct:isPartOf F2021L00308:36 ;
    dct:isReferencedBy F2021L00308: ;
    rdfs:comment "4 9  Areas for preparation of prescribed ratite meat or ratite meat products - Abrievated Graph Key: I45"@en-AU ;
    skos:definition "4 9  Areas for preparation of prescribed ratite meat or ratite meat products"@en-AU ;
    skos:narrower F2021L00308:36 ;
    skos:prefLabel "Item I45"@en-AU ;
    dcat:accessURL <https://www.legislation.gov.au/F2021L00308/2023-08-04/2023-08-04/text/original/epub/OEBPS/document_1/document_1.html#_Toc143604754> ;
    dcat:landingPage "https://www.legislation.gov.au/F2021L00308/2023-08-04/2023-08-04/text/original/epub/OEBPS/document_1/document_1.html#_Toc143604754"^^xsd:anyURI ;
    dcat:theme legcons:Item .

F2021L00308:46 a legcons:Item,
        owl:Class,
        dcat:Resource ;
    rdfs:label "Item - I46 4 10  Secure storage area"@en-AU ;
    dct:isPartOf F2021L00308:36 ;
    dct:isReferencedBy F2021L00308: ;
    rdfs:comment "4 10  Secure storage area - Abrievated Graph Key: I46"@en-AU ;
    skos:definition "4 10  Secure storage area"@en-AU ;
    skos:narrower F2021L00308:36 ;
    skos:prefLabel "Item I46"@en-AU ;
    dcat:accessURL <https://www.legislation.gov.au/F2021L00308/2023-08-04/2023-08-04/text/original/epub/OEBPS/document_1/document_1.html#_Toc143604755> ;
    dcat:landingPage "https://www.legislation.gov.au/F2021L00308/2023-08-04/2023-08-04/text/original/epub/OEBPS/document_1/document_1.html#_Toc143604755"^^xsd:anyURI ;
    dcat:theme legcons:Item .

F2021L00308:47 a legcons:Item,
        owl:Class,
        dcat:Resource ;
    rdfs:label "Item - I47 4 11  Amenities for Commonwealth authorised officers"@en-AU ;
    dct:isPartOf F2021L00308:36 ;
    dct:isReferencedBy F2021L00308: ;
    rdfs:comment "4 11  Amenities for Commonwealth authorised officers - Abrievated Graph Key: I47"@en-AU ;
    skos:definition "4 11  Amenities for Commonwealth authorised officers"@en-AU ;
    skos:narrower F2021L00308:36 ;
    skos:prefLabel "Item I47"@en-AU ;
    dcat:accessURL <https://www.legislation.gov.au/F2021L00308/2023-08-04/2023-08-04/text/original/epub/OEBPS/document_1/document_1.html#_Toc143604756> ;
    dcat:landingPage "https://www.legislation.gov.au/F2021L00308/2023-08-04/2023-08-04/text/original/epub/OEBPS/document_1/document_1.html#_Toc143604756"^^xsd:anyURI ;
    dcat:theme legcons:Item .

F2021L00308:49 a legcons:Item,
        owl:Class,
        dcat:Resource ;
    rdfs:label "Item - I49 4 12  Purpose of this Part"@en-AU ;
    dct:isPartOf F2021L00308:48 ;
    dct:isReferencedBy F2021L00308: ;
    rdfs:comment "4 12  Purpose of this Part - Abrievated Graph Key: I49"@en-AU ;
    skos:definition "4 12  Purpose of this Part"@en-AU ;
    skos:narrower F2021L00308:48 ;
    skos:prefLabel "Item I49"@en-AU ;
    dcat:accessURL <https://www.legislation.gov.au/F2021L00308/2023-08-04/2023-08-04/text/original/epub/OEBPS/document_1/document_1.html#_Toc143604758> ;
    dcat:landingPage "https://www.legislation.gov.au/F2021L00308/2023-08-04/2023-08-04/text/original/epub/OEBPS/document_1/document_1.html#_Toc143604758"^^xsd:anyURI ;
    dcat:theme legcons:Item .

F2021L00308:5 a legcons:Item,
        owl:Class,
        dcat:Resource ;
    rdfs:label "Item - I5 1 4  Simplified outline of this instrument"@en-AU ;
    dct:isPartOf F2021L00308:1 ;
    dct:isReferencedBy F2021L00308: ;
    rdfs:comment "1 4  Simplified outline of this instrument - Abrievated Graph Key: I5"@en-AU ;
    skos:definition "1 4  Simplified outline of this instrument"@en-AU ;
    skos:narrower F2021L00308:1 ;
    skos:prefLabel "Item I5"@en-AU ;
    dcat:accessURL <https://www.legislation.gov.au/F2021L00308/2023-08-04/2023-08-04/text/original/epub/OEBPS/document_1/document_1.html#_Toc143604714> ;
    dcat:landingPage "https://www.legislation.gov.au/F2021L00308/2023-08-04/2023-08-04/text/original/epub/OEBPS/document_1/document_1.html#_Toc143604714"^^xsd:anyURI ;
    dcat:theme legcons:Item .

F2021L00308:50 a legcons:Item,
        owl:Class,
        dcat:Resource ;
    rdfs:label "Item - I50 4 13  Requirements for registration continue to be met"@en-AU ;
    dct:isPartOf F2021L00308:48 ;
    dct:isReferencedBy F2021L00308: ;
    rdfs:comment "4 13  Requirements for registration continue to be met - Abrievated Graph Key: I50"@en-AU ;
    skos:definition "4 13  Requirements for registration continue to be met"@en-AU ;
    skos:narrower F2021L00308:48 ;
    skos:prefLabel "Item I50"@en-AU ;
    dcat:accessURL <https://www.legislation.gov.au/F2021L00308/2023-08-04/2023-08-04/text/original/epub/OEBPS/document_1/document_1.html#_Toc143604759> ;
    dcat:landingPage "https://www.legislation.gov.au/F2021L00308/2023-08-04/2023-08-04/text/original/epub/OEBPS/document_1/document_1.html#_Toc143604759"^^xsd:anyURI ;
    dcat:theme legcons:Item .

F2021L00308:51 a legcons:Item,
        owl:Class,
        dcat:Resource ;
    rdfs:label "Item - I51 4 14  Certificate of registration must be displayed"@en-AU ;
    dct:isPartOf F2021L00308:48 ;
    dct:isReferencedBy F2021L00308: ;
    rdfs:comment "4 14  Certificate of registration must be displayed - Abrievated Graph Key: I51"@en-AU ;
    skos:definition "4 14  Certificate of registration must be displayed"@en-AU ;
    skos:narrower F2021L00308:48 ;
    skos:prefLabel "Item I51"@en-AU ;
    dcat:accessURL <https://www.legislation.gov.au/F2021L00308/2023-08-04/2023-08-04/text/original/epub/OEBPS/document_1/document_1.html#_Toc143604760> ;
    dcat:landingPage "https://www.legislation.gov.au/F2021L00308/2023-08-04/2023-08-04/text/original/epub/OEBPS/document_1/document_1.html#_Toc143604760"^^xsd:anyURI ;
    dcat:theme legcons:Item .

F2021L00308:52 a legcons:Item,
        owl:Class,
        dcat:Resource ;
    rdfs:label "Item - I52 4 15  Notice of certain matters must be given to persons who manage or control export operations at registered establishment"@en-AU ;
    dct:isPartOf F2021L00308:48 ;
    dct:isReferencedBy F2021L00308: ;
    rdfs:comment "4 15  Notice of certain matters must be given to persons who manage or control export operations at registered establishment - Abrievated Graph Key: I52"@en-AU ;
    skos:definition "4 15  Notice of certain matters must be given to persons who manage or control export operations at registered establishment"@en-AU ;
    skos:narrower F2021L00308:48 ;
    skos:prefLabel "Item I52"@en-AU ;
    dcat:accessURL <https://www.legislation.gov.au/F2021L00308/2023-08-04/2023-08-04/text/original/epub/OEBPS/document_1/document_1.html#_Toc143604761> ;
    dcat:landingPage "https://www.legislation.gov.au/F2021L00308/2023-08-04/2023-08-04/text/original/epub/OEBPS/document_1/document_1.html#_Toc143604761"^^xsd:anyURI ;
    dcat:theme legcons:Item .

F2021L00308:53 a legcons:Item,
        owl:Class,
        dcat:Resource ;
    rdfs:label "Item - I53 4 16  List of persons who manage or control export operations at registered establishment"@en-AU ;
    dct:isPartOf F2021L00308:48 ;
    dct:isReferencedBy F2021L00308: ;
    rdfs:comment "4 16  List of persons who manage or control export operations at registered establishment - Abrievated Graph Key: I53"@en-AU ;
    skos:definition "4 16  List of persons who manage or control export operations at registered establishment"@en-AU ;
    skos:narrower F2021L00308:48 ;
    skos:prefLabel "Item I53"@en-AU ;
    dcat:accessURL <https://www.legislation.gov.au/F2021L00308/2023-08-04/2023-08-04/text/original/epub/OEBPS/document_1/document_1.html#_Toc143604762> ;
    dcat:landingPage "https://www.legislation.gov.au/F2021L00308/2023-08-04/2023-08-04/text/original/epub/OEBPS/document_1/document_1.html#_Toc143604762"^^xsd:anyURI ;
    dcat:theme legcons:Item .

F2021L00308:54 a legcons:Item,
        owl:Class,
        dcat:Resource ;
    rdfs:label "Item - I54 4 17  Meat inspection services"@en-AU ;
    dct:isPartOf F2021L00308:48 ;
    dct:isReferencedBy F2021L00308: ;
    rdfs:comment "4 17  Meat inspection services - Abrievated Graph Key: I54"@en-AU ;
    skos:definition "4 17  Meat inspection services"@en-AU ;
    skos:narrower F2021L00308:48 ;
    skos:prefLabel "Item I54"@en-AU ;
    dcat:accessURL <https://www.legislation.gov.au/F2021L00308/2023-08-04/2023-08-04/text/original/epub/OEBPS/document_1/document_1.html#_Toc143604763> ;
    dcat:landingPage "https://www.legislation.gov.au/F2021L00308/2023-08-04/2023-08-04/text/original/epub/OEBPS/document_1/document_1.html#_Toc143604763"^^xsd:anyURI ;
    dcat:theme legcons:Item .

F2021L00308:56 a legcons:Item,
        owl:Class,
        dcat:Resource ;
    rdfs:label "Item - I56 4 18  Period within which application to renew registration must be made"@en-AU ;
    dct:isPartOf F2021L00308:55 ;
    dct:isReferencedBy F2021L00308: ;
    rdfs:comment "4 18  Period within which application to renew registration must be made - Abrievated Graph Key: I56"@en-AU ;
    skos:definition "4 18  Period within which application to renew registration must be made"@en-AU ;
    skos:narrower F2021L00308:55 ;
    skos:prefLabel "Item I56"@en-AU ;
    dcat:accessURL <https://www.legislation.gov.au/F2021L00308/2023-08-04/2023-08-04/text/original/epub/OEBPS/document_1/document_1.html#_Toc143604765> ;
    dcat:landingPage "https://www.legislation.gov.au/F2021L00308/2023-08-04/2023-08-04/text/original/epub/OEBPS/document_1/document_1.html#_Toc143604765"^^xsd:anyURI ;
    dcat:theme legcons:Item .

F2021L00308:57 a legcons:Item,
        owl:Class,
        dcat:Resource ;
    rdfs:label "Item - I57 4 19  Requirements for renewal of registration"@en-AU ;
    dct:isPartOf F2021L00308:55 ;
    dct:isReferencedBy F2021L00308: ;
    rdfs:comment "4 19  Requirements for renewal of registration - Abrievated Graph Key: I57"@en-AU ;
    skos:definition "4 19  Requirements for renewal of registration"@en-AU ;
    skos:narrower F2021L00308:55 ;
    skos:prefLabel "Item I57"@en-AU ;
    dcat:accessURL <https://www.legislation.gov.au/F2021L00308/2023-08-04/2023-08-04/text/original/epub/OEBPS/document_1/document_1.html#_Toc143604766> ;
    dcat:landingPage "https://www.legislation.gov.au/F2021L00308/2023-08-04/2023-08-04/text/original/epub/OEBPS/document_1/document_1.html#_Toc143604766"^^xsd:anyURI ;
    dcat:theme legcons:Item .

F2021L00308:59 a legcons:Item,
        owl:Class,
        dcat:Resource ;
    rdfs:label "Item - I59 4 20  Alterations for which approval is not required"@en-AU ;
    dct:isPartOf F2021L00308:58 ;
    dct:isReferencedBy F2021L00308: ;
    rdfs:comment "4 20  Alterations for which approval is not required - Abrievated Graph Key: I59"@en-AU ;
    skos:definition "4 20  Alterations for which approval is not required"@en-AU ;
    skos:narrower F2021L00308:58 ;
    skos:prefLabel "Item I59"@en-AU ;
    dcat:accessURL <https://www.legislation.gov.au/F2021L00308/2023-08-04/2023-08-04/text/original/epub/OEBPS/document_1/document_1.html#_Toc143604768> ;
    dcat:landingPage "https://www.legislation.gov.au/F2021L00308/2023-08-04/2023-08-04/text/original/epub/OEBPS/document_1/document_1.html#_Toc143604768"^^xsd:anyURI ;
    dcat:theme legcons:Item .

F2021L00308:6 a legcons:Part,
        owl:Class,
        dcat:Resource ;
    rdfs:label "Part - P6 Part 2 Interpretation"@en-AU ;
    dct:isPartOf F2021L00308:1 ;
    dct:isReferencedBy F2021L00308: ;
    rdfs:comment "Part 2 Interpretation - Abrievated Graph Key: P6"@en-AU ;
    skos:definition "Part 2 Interpretation"@en-AU ;
    skos:narrower F2021L00308:1 ;
    skos:prefLabel "Part P6"@en-AU ;
    dcat:accessURL <https://www.legislation.gov.au/F2021L00308/2023-08-04/2023-08-04/text/original/epub/OEBPS/document_1/document_1.html#_Toc143604715> ;
    dcat:landingPage "https://www.legislation.gov.au/F2021L00308/2023-08-04/2023-08-04/text/original/epub/OEBPS/document_1/document_1.html#_Toc143604715"^^xsd:anyURI ;
    dcat:theme legcons:Part .

F2021L00308:61 a legcons:Item,
        owl:Class,
        dcat:Resource ;
    rdfs:label "Item - I61 4 21  Application of this Part"@en-AU ;
    dct:isPartOf F2021L00308:60 ;
    dct:isReferencedBy F2021L00308: ;
    rdfs:comment "4 21  Application of this Part - Abrievated Graph Key: I61"@en-AU ;
    skos:definition "4 21  Application of this Part"@en-AU ;
    skos:narrower F2021L00308:60 ;
    skos:prefLabel "Item I61"@en-AU ;
    dcat:accessURL <https://www.legislation.gov.au/F2021L00308/2023-08-04/2023-08-04/text/original/epub/OEBPS/document_1/document_1.html#_Toc143604770> ;
    dcat:landingPage "https://www.legislation.gov.au/F2021L00308/2023-08-04/2023-08-04/text/original/epub/OEBPS/document_1/document_1.html#_Toc143604770"^^xsd:anyURI ;
    dcat:theme legcons:Item .

F2021L00308:62 a legcons:Item,
        owl:Class,
        dcat:Resource ;
    rdfs:label "Item - I62 4 22  Initial consideration period"@en-AU ;
    dct:isPartOf F2021L00308:60 ;
    dct:isReferencedBy F2021L00308: ;
    rdfs:comment "4 22  Initial consideration period - Abrievated Graph Key: I62"@en-AU ;
    skos:definition "4 22  Initial consideration period"@en-AU ;
    skos:narrower F2021L00308:60 ;
    skos:prefLabel "Item I62"@en-AU ;
    dcat:accessURL <https://www.legislation.gov.au/F2021L00308/2023-08-04/2023-08-04/text/original/epub/OEBPS/document_1/document_1.html#_Toc143604771> ;
    dcat:landingPage "https://www.legislation.gov.au/F2021L00308/2023-08-04/2023-08-04/text/original/epub/OEBPS/document_1/document_1.html#_Toc143604771"^^xsd:anyURI ;
    dcat:theme legcons:Item .

F2021L00308:63 a legcons:Item,
        owl:Class,
        dcat:Resource ;
    rdfs:label "Item - I63 4 23  Period within which request relating to application must be complied with"@en-AU ;
    dct:isPartOf F2021L00308:60 ;
    dct:isReferencedBy F2021L00308: ;
    rdfs:comment "4 23  Period within which request relating to application must be complied with - Abrievated Graph Key: I63"@en-AU ;
    skos:definition "4 23  Period within which request relating to application must be complied with"@en-AU ;
    skos:narrower F2021L00308:60 ;
    skos:prefLabel "Item I63"@en-AU ;
    dcat:accessURL <https://www.legislation.gov.au/F2021L00308/2023-08-04/2023-08-04/text/original/epub/OEBPS/document_1/document_1.html#_Toc143604772> ;
    dcat:landingPage "https://www.legislation.gov.au/F2021L00308/2023-08-04/2023-08-04/text/original/epub/OEBPS/document_1/document_1.html#_Toc143604772"^^xsd:anyURI ;
    dcat:theme legcons:Item .

F2021L00308:66 a legcons:Item,
        owl:Class,
        dcat:Resource ;
    rdfs:label "Item - I66 4 24  Application for allocation of meat inspection services to establishment"@en-AU ;
    dct:isPartOf F2021L00308:65 ;
    dct:isReferencedBy F2021L00308: ;
    rdfs:comment "4 24  Application for allocation of meat inspection services to establishment - Abrievated Graph Key: I66"@en-AU ;
    skos:definition "4 24  Application for allocation of meat inspection services to establishment"@en-AU ;
    skos:narrower F2021L00308:65 ;
    skos:prefLabel "Item I66"@en-AU ;
    dcat:accessURL <https://www.legislation.gov.au/F2021L00308/2023-08-04/2023-08-04/text/original/epub/OEBPS/document_1/document_1.html#_Toc143604775> ;
    dcat:landingPage "https://www.legislation.gov.au/F2021L00308/2023-08-04/2023-08-04/text/original/epub/OEBPS/document_1/document_1.html#_Toc143604775"^^xsd:anyURI ;
    dcat:theme legcons:Item .

F2021L00308:67 a legcons:Item,
        owl:Class,
        dcat:Resource ;
    rdfs:label "Item - I67 4 25  Preliminary allocation"@en-AU ;
    dct:isPartOf F2021L00308:65 ;
    dct:isReferencedBy F2021L00308: ;
    rdfs:comment "4 25  Preliminary allocation - Abrievated Graph Key: I67"@en-AU ;
    skos:definition "4 25  Preliminary allocation"@en-AU ;
    skos:narrower F2021L00308:65 ;
    skos:prefLabel "Item I67"@en-AU ;
    dcat:accessURL <https://www.legislation.gov.au/F2021L00308/2023-08-04/2023-08-04/text/original/epub/OEBPS/document_1/document_1.html#_Toc143604776> ;
    dcat:landingPage "https://www.legislation.gov.au/F2021L00308/2023-08-04/2023-08-04/text/original/epub/OEBPS/document_1/document_1.html#_Toc143604776"^^xsd:anyURI ;
    dcat:theme legcons:Item .

F2021L00308:68 a legcons:Item,
        owl:Class,
        dcat:Resource ;
    rdfs:label "Item - I68 4 26  Notice of preliminary allocation"@en-AU ;
    dct:isPartOf F2021L00308:65 ;
    dct:isReferencedBy F2021L00308: ;
    rdfs:comment "4 26  Notice of preliminary allocation - Abrievated Graph Key: I68"@en-AU ;
    skos:definition "4 26  Notice of preliminary allocation"@en-AU ;
    skos:narrower F2021L00308:65 ;
    skos:prefLabel "Item I68"@en-AU ;
    dcat:accessURL <https://www.legislation.gov.au/F2021L00308/2023-08-04/2023-08-04/text/original/epub/OEBPS/document_1/document_1.html#_Toc143604777> ;
    dcat:landingPage "https://www.legislation.gov.au/F2021L00308/2023-08-04/2023-08-04/text/original/epub/OEBPS/document_1/document_1.html#_Toc143604777"^^xsd:anyURI ;
    dcat:theme legcons:Item .

F2021L00308:69 a legcons:Item,
        owl:Class,
        dcat:Resource ;
    rdfs:label "Item - I69 4 27  Procedure following notice of preliminary allocation"@en-AU ;
    dct:isPartOf F2021L00308:65 ;
    dct:isReferencedBy F2021L00308: ;
    rdfs:comment "4 27  Procedure following notice of preliminary allocation - Abrievated Graph Key: I69"@en-AU ;
    skos:definition "4 27  Procedure following notice of preliminary allocation"@en-AU ;
    skos:narrower F2021L00308:65 ;
    skos:prefLabel "Item I69"@en-AU ;
    dcat:accessURL <https://www.legislation.gov.au/F2021L00308/2023-08-04/2023-08-04/text/original/epub/OEBPS/document_1/document_1.html#_Toc143604778> ;
    dcat:landingPage "https://www.legislation.gov.au/F2021L00308/2023-08-04/2023-08-04/text/original/epub/OEBPS/document_1/document_1.html#_Toc143604778"^^xsd:anyURI ;
    dcat:theme legcons:Item .

F2021L00308:7 a legcons:Division,
        owl:Class,
        dcat:Resource ;
    rdfs:label "Division - D7 Division 1 Definitions"@en-AU ;
    dct:isPartOf F2021L00308:1 ;
    dct:isReferencedBy F2021L00308: ;
    rdfs:comment "Division 1 Definitions - Abrievated Graph Key: D7"@en-AU ;
    skos:definition "Division 1 Definitions"@en-AU ;
    skos:narrower F2021L00308:1 ;
    skos:prefLabel "Division D7"@en-AU ;
    dcat:accessURL <https://www.legislation.gov.au/F2021L00308/2023-08-04/2023-08-04/text/original/epub/OEBPS/document_1/document_1.html#_Toc143604716> ;
    dcat:landingPage "https://www.legislation.gov.au/F2021L00308/2023-08-04/2023-08-04/text/original/epub/OEBPS/document_1/document_1.html#_Toc143604716"^^xsd:anyURI ;
    dcat:theme legcons:Division .

F2021L00308:70 a legcons:Item,
        owl:Class,
        dcat:Resource ;
    rdfs:label "Item - I70 4 28  Revised allocation"@en-AU ;
    dct:isPartOf F2021L00308:65 ;
    dct:isReferencedBy F2021L00308: ;
    rdfs:comment "4 28  Revised allocation - Abrievated Graph Key: I70"@en-AU ;
    skos:definition "4 28  Revised allocation"@en-AU ;
    skos:narrower F2021L00308:65 ;
    skos:prefLabel "Item I70"@en-AU ;
    dcat:accessURL <https://www.legislation.gov.au/F2021L00308/2023-08-04/2023-08-04/text/original/epub/OEBPS/document_1/document_1.html#_Toc143604779> ;
    dcat:landingPage "https://www.legislation.gov.au/F2021L00308/2023-08-04/2023-08-04/text/original/epub/OEBPS/document_1/document_1.html#_Toc143604779"^^xsd:anyURI ;
    dcat:theme legcons:Item .

F2021L00308:71 a legcons:Item,
        owl:Class,
        dcat:Resource ;
    rdfs:label "Item - I71 4 29  Procedure following notice of revised allocation"@en-AU ;
    dct:isPartOf F2021L00308:65 ;
    dct:isReferencedBy F2021L00308: ;
    rdfs:comment "4 29  Procedure following notice of revised allocation - Abrievated Graph Key: I71"@en-AU ;
    skos:definition "4 29  Procedure following notice of revised allocation"@en-AU ;
    skos:narrower F2021L00308:65 ;
    skos:prefLabel "Item I71"@en-AU ;
    dcat:accessURL <https://www.legislation.gov.au/F2021L00308/2023-08-04/2023-08-04/text/original/epub/OEBPS/document_1/document_1.html#_Toc143604780> ;
    dcat:landingPage "https://www.legislation.gov.au/F2021L00308/2023-08-04/2023-08-04/text/original/epub/OEBPS/document_1/document_1.html#_Toc143604780"^^xsd:anyURI ;
    dcat:theme legcons:Item .

F2021L00308:72 a legcons:Item,
        owl:Class,
        dcat:Resource ;
    rdfs:label "Item - I72 4 30  Review of Secretarys determination"@en-AU ;
    dct:isPartOf F2021L00308:65 ;
    dct:isReferencedBy F2021L00308: ;
    rdfs:comment "4 30  Review of Secretarys determination - Abrievated Graph Key: I72"@en-AU ;
    skos:definition "4 30  Review of Secretarys determination"@en-AU ;
    skos:narrower F2021L00308:65 ;
    skos:prefLabel "Item I72"@en-AU ;
    dcat:accessURL <https://www.legislation.gov.au/F2021L00308/2023-08-04/2023-08-04/text/original/epub/OEBPS/document_1/document_1.html#_Toc143604781> ;
    dcat:landingPage "https://www.legislation.gov.au/F2021L00308/2023-08-04/2023-08-04/text/original/epub/OEBPS/document_1/document_1.html#_Toc143604781"^^xsd:anyURI ;
    dcat:theme legcons:Item .

F2021L00308:73 a legcons:Item,
        owl:Class,
        dcat:Resource ;
    rdfs:label "Item - I73 4 31  Determination of new allocation"@en-AU ;
    dct:isPartOf F2021L00308:65 ;
    dct:isReferencedBy F2021L00308: ;
    rdfs:comment "4 31  Determination of new allocation - Abrievated Graph Key: I73"@en-AU ;
    skos:definition "4 31  Determination of new allocation"@en-AU ;
    skos:narrower F2021L00308:65 ;
    skos:prefLabel "Item I73"@en-AU ;
    dcat:accessURL <https://www.legislation.gov.au/F2021L00308/2023-08-04/2023-08-04/text/original/epub/OEBPS/document_1/document_1.html#_Toc143604782> ;
    dcat:landingPage "https://www.legislation.gov.au/F2021L00308/2023-08-04/2023-08-04/text/original/epub/OEBPS/document_1/document_1.html#_Toc143604782"^^xsd:anyURI ;
    dcat:theme legcons:Item .

F2021L00308:75 a legcons:Item,
        owl:Class,
        dcat:Resource ;
    rdfs:label "Item - I75 4 32  Application to vary allocation of meat inspection services"@en-AU ;
    dct:isPartOf F2021L00308:74 ;
    dct:isReferencedBy F2021L00308: ;
    rdfs:comment "4 32  Application to vary allocation of meat inspection services - Abrievated Graph Key: I75"@en-AU ;
    skos:definition "4 32  Application to vary allocation of meat inspection services"@en-AU ;
    skos:narrower F2021L00308:74 ;
    skos:prefLabel "Item I75"@en-AU ;
    dcat:accessURL <https://www.legislation.gov.au/F2021L00308/2023-08-04/2023-08-04/text/original/epub/OEBPS/document_1/document_1.html#_Toc143604784> ;
    dcat:landingPage "https://www.legislation.gov.au/F2021L00308/2023-08-04/2023-08-04/text/original/epub/OEBPS/document_1/document_1.html#_Toc143604784"^^xsd:anyURI ;
    dcat:theme legcons:Item .

F2021L00308:76 a legcons:Item,
        owl:Class,
        dcat:Resource ;
    rdfs:label "Item - I76 4 33  Application for additional allocation of meat inspection services"@en-AU ;
    dct:isPartOf F2021L00308:74 ;
    dct:isReferencedBy F2021L00308: ;
    rdfs:comment "4 33  Application for additional allocation of meat inspection services - Abrievated Graph Key: I76"@en-AU ;
    skos:definition "4 33  Application for additional allocation of meat inspection services"@en-AU ;
    skos:narrower F2021L00308:74 ;
    skos:prefLabel "Item I76"@en-AU ;
    dcat:accessURL <https://www.legislation.gov.au/F2021L00308/2023-08-04/2023-08-04/text/original/epub/OEBPS/document_1/document_1.html#_Toc143604785> ;
    dcat:landingPage "https://www.legislation.gov.au/F2021L00308/2023-08-04/2023-08-04/text/original/epub/OEBPS/document_1/document_1.html#_Toc143604785"^^xsd:anyURI ;
    dcat:theme legcons:Item .

F2021L00308:77 a legcons:Item,
        owl:Class,
        dcat:Resource ;
    rdfs:label "Item - I77 4 34  Notification that meat inspection services not required during shutdown period"@en-AU ;
    dct:isPartOf F2021L00308:74 ;
    dct:isReferencedBy F2021L00308: ;
    rdfs:comment "4 34  Notification that meat inspection services not required during shutdown period - Abrievated Graph Key: I77"@en-AU ;
    skos:definition "4 34  Notification that meat inspection services not required during shutdown period"@en-AU ;
    skos:narrower F2021L00308:74 ;
    skos:prefLabel "Item I77"@en-AU ;
    dcat:accessURL <https://www.legislation.gov.au/F2021L00308/2023-08-04/2023-08-04/text/original/epub/OEBPS/document_1/document_1.html#_Toc143604786> ;
    dcat:landingPage "https://www.legislation.gov.au/F2021L00308/2023-08-04/2023-08-04/text/original/epub/OEBPS/document_1/document_1.html#_Toc143604786"^^xsd:anyURI ;
    dcat:theme legcons:Item .

F2021L00308:78 a legcons:Item,
        owl:Class,
        dcat:Resource ;
    rdfs:label "Item - I78 4 35  Variation by Secretary of allocation of meat inspection services"@en-AU ;
    dct:isPartOf F2021L00308:74 ;
    dct:isReferencedBy F2021L00308: ;
    rdfs:comment "4 35  Variation by Secretary of allocation of meat inspection services - Abrievated Graph Key: I78"@en-AU ;
    skos:definition "4 35  Variation by Secretary of allocation of meat inspection services"@en-AU ;
    skos:narrower F2021L00308:74 ;
    skos:prefLabel "Item I78"@en-AU ;
    dcat:accessURL <https://www.legislation.gov.au/F2021L00308/2023-08-04/2023-08-04/text/original/epub/OEBPS/document_1/document_1.html#_Toc143604787> ;
    dcat:landingPage "https://www.legislation.gov.au/F2021L00308/2023-08-04/2023-08-04/text/original/epub/OEBPS/document_1/document_1.html#_Toc143604787"^^xsd:anyURI ;
    dcat:theme legcons:Item .

F2021L00308:79 a legcons:Item,
        owl:Class,
        dcat:Resource ;
    rdfs:label "Item - I79 4 36  Notification of termination of meat inspection services"@en-AU ;
    dct:isPartOf F2021L00308:74 ;
    dct:isReferencedBy F2021L00308: ;
    rdfs:comment "4 36  Notification of termination of meat inspection services - Abrievated Graph Key: I79"@en-AU ;
    skos:definition "4 36  Notification of termination of meat inspection services"@en-AU ;
    skos:narrower F2021L00308:74 ;
    skos:prefLabel "Item I79"@en-AU ;
    dcat:accessURL <https://www.legislation.gov.au/F2021L00308/2023-08-04/2023-08-04/text/original/epub/OEBPS/document_1/document_1.html#_Toc143604788> ;
    dcat:landingPage "https://www.legislation.gov.au/F2021L00308/2023-08-04/2023-08-04/text/original/epub/OEBPS/document_1/document_1.html#_Toc143604788"^^xsd:anyURI ;
    dcat:theme legcons:Item .

F2021L00308:8 a legcons:Item,
        owl:Class,
        dcat:Resource ;
    rdfs:label "Item - I8 1 5  Definitions"@en-AU ;
    dct:isPartOf F2021L00308:1 ;
    dct:isReferencedBy F2021L00308: ;
    rdfs:comment "1 5  Definitions - Abrievated Graph Key: I8"@en-AU ;
    skos:definition "1 5  Definitions"@en-AU ;
    skos:narrower F2021L00308:1 ;
    skos:prefLabel "Item I8"@en-AU ;
    dcat:accessURL <https://www.legislation.gov.au/F2021L00308/2023-08-04/2023-08-04/text/original/epub/OEBPS/document_1/document_1.html#_Toc143604717> ;
    dcat:landingPage "https://www.legislation.gov.au/F2021L00308/2023-08-04/2023-08-04/text/original/epub/OEBPS/document_1/document_1.html#_Toc143604717"^^xsd:anyURI ;
    dcat:theme legcons:Item .

F2021L00308:82 a legcons:Item,
        owl:Class,
        dcat:Resource ;
    rdfs:label "Item - I82 5 1  Purpose of this Part"@en-AU ;
    dct:isPartOf F2021L00308:81 ;
    dct:isReferencedBy F2021L00308: ;
    rdfs:comment "5 1  Purpose of this Part - Abrievated Graph Key: I82"@en-AU ;
    skos:definition "5 1  Purpose of this Part"@en-AU ;
    skos:narrower F2021L00308:81 ;
    skos:prefLabel "Item I82"@en-AU ;
    dcat:accessURL <https://www.legislation.gov.au/F2021L00308/2023-08-04/2023-08-04/text/original/epub/OEBPS/document_1/document_1.html#_Toc143604791> ;
    dcat:landingPage "https://www.legislation.gov.au/F2021L00308/2023-08-04/2023-08-04/text/original/epub/OEBPS/document_1/document_1.html#_Toc143604791"^^xsd:anyURI ;
    dcat:theme legcons:Item .

F2021L00308:83 a legcons:Item,
        owl:Class,
        dcat:Resource ;
    rdfs:label "Item - I83 5 2  Other requirementsproposed arrangement for operations to prepare prescribed rabbit meat ratite meat rabbit meat products or ratite meat products"@en-AU ;
    dct:isPartOf F2021L00308:81 ;
    dct:isReferencedBy F2021L00308: ;
    rdfs:comment "5 2  Other requirementsproposed arrangement for operations to prepare prescribed rabbit meat ratite meat rabbit meat products or ratite meat products - Abrievated Graph Key: I83"@en-AU ;
    skos:definition "5 2  Other requirementsproposed arrangement for operations to prepare prescribed rabbit meat ratite meat rabbit meat products or ratite meat products"@en-AU ;
    skos:narrower F2021L00308:81 ;
    skos:prefLabel "Item I83"@en-AU ;
    dcat:accessURL <https://www.legislation.gov.au/F2021L00308/2023-08-04/2023-08-04/text/original/epub/OEBPS/document_1/document_1.html#_Toc143604792> ;
    dcat:landingPage "https://www.legislation.gov.au/F2021L00308/2023-08-04/2023-08-04/text/original/epub/OEBPS/document_1/document_1.html#_Toc143604792"^^xsd:anyURI ;
    dcat:theme legcons:Item .

F2021L00308:86 a legcons:Item,
        owl:Class,
        dcat:Resource ;
    rdfs:label "Item - I86 5 3  Purpose of this Part"@en-AU ;
    dct:isPartOf F2021L00308:85 ;
    dct:isReferencedBy F2021L00308: ;
    rdfs:comment "5 3  Purpose of this Part - Abrievated Graph Key: I86"@en-AU ;
    skos:definition "5 3  Purpose of this Part"@en-AU ;
    skos:narrower F2021L00308:85 ;
    skos:prefLabel "Item I86"@en-AU ;
    dcat:accessURL <https://www.legislation.gov.au/F2021L00308/2023-08-04/2023-08-04/text/original/epub/OEBPS/document_1/document_1.html#_Toc143604795> ;
    dcat:landingPage "https://www.legislation.gov.au/F2021L00308/2023-08-04/2023-08-04/text/original/epub/OEBPS/document_1/document_1.html#_Toc143604795"^^xsd:anyURI ;
    dcat:theme legcons:Item .

F2021L00308:88 a legcons:Item,
        owl:Class,
        dcat:Resource ;
    rdfs:label "Item - I88 5 4  Importing country requirements must be met"@en-AU ;
    dct:isPartOf F2021L00308:87 ;
    dct:isReferencedBy F2021L00308: ;
    rdfs:comment "5 4  Importing country requirements must be met - Abrievated Graph Key: I88"@en-AU ;
    skos:definition "5 4  Importing country requirements must be met"@en-AU ;
    skos:narrower F2021L00308:87 ;
    skos:prefLabel "Item I88"@en-AU ;
    dcat:accessURL <https://www.legislation.gov.au/F2021L00308/2023-08-04/2023-08-04/text/original/epub/OEBPS/document_1/document_1.html#_Toc143604797> ;
    dcat:landingPage "https://www.legislation.gov.au/F2021L00308/2023-08-04/2023-08-04/text/original/epub/OEBPS/document_1/document_1.html#_Toc143604797"^^xsd:anyURI ;
    dcat:theme legcons:Item .

F2021L00308:89 a legcons:Item,
        owl:Class,
        dcat:Resource ;
    rdfs:label "Item - I89 5 5  Requirements of Australian Meat Standard must be met"@en-AU ;
    dct:isPartOf F2021L00308:87 ;
    dct:isReferencedBy F2021L00308: ;
    rdfs:comment "5 5  Requirements of Australian Meat Standard must be met - Abrievated Graph Key: I89"@en-AU ;
    skos:definition "5 5  Requirements of Australian Meat Standard must be met"@en-AU ;
    skos:narrower F2021L00308:87 ;
    skos:prefLabel "Item I89"@en-AU ;
    dcat:accessURL <https://www.legislation.gov.au/F2021L00308/2023-08-04/2023-08-04/text/original/epub/OEBPS/document_1/document_1.html#_Toc143604798> ;
    dcat:landingPage "https://www.legislation.gov.au/F2021L00308/2023-08-04/2023-08-04/text/original/epub/OEBPS/document_1/document_1.html#_Toc143604798"^^xsd:anyURI ;
    dcat:theme legcons:Item .

F2021L00308:9 a legcons:Item,
        owl:Class,
        dcat:Resource ;
    rdfs:label "Item - I9 1 6  Meaning of loaded for export"@en-AU ;
    dct:isPartOf F2021L00308:1 ;
    dct:isReferencedBy F2021L00308: ;
    rdfs:comment "1 6  Meaning of loaded for export - Abrievated Graph Key: I9"@en-AU ;
    skos:definition "1 6  Meaning of loaded for export"@en-AU ;
    skos:narrower F2021L00308:1 ;
    skos:prefLabel "Item I9"@en-AU ;
    dcat:accessURL <https://www.legislation.gov.au/F2021L00308/2023-08-04/2023-08-04/text/original/epub/OEBPS/document_1/document_1.html#_Toc143604718> ;
    dcat:landingPage "https://www.legislation.gov.au/F2021L00308/2023-08-04/2023-08-04/text/original/epub/OEBPS/document_1/document_1.html#_Toc143604718"^^xsd:anyURI ;
    dcat:theme legcons:Item .

F2021L00308:92 a legcons:Item,
        owl:Class,
        dcat:Resource ;
    rdfs:label "Item - I92 5 6  Dressing an animal"@en-AU ;
    dct:isPartOf F2021L00308:91 ;
    dct:isReferencedBy F2021L00308: ;
    rdfs:comment "5 6  Dressing an animal - Abrievated Graph Key: I92"@en-AU ;
    skos:definition "5 6  Dressing an animal"@en-AU ;
    skos:narrower F2021L00308:91 ;
    skos:prefLabel "Item I92"@en-AU ;
    dcat:accessURL <https://www.legislation.gov.au/F2021L00308/2023-08-04/2023-08-04/text/original/epub/OEBPS/document_1/document_1.html#_Toc143604801> ;
    dcat:landingPage "https://www.legislation.gov.au/F2021L00308/2023-08-04/2023-08-04/text/original/epub/OEBPS/document_1/document_1.html#_Toc143604801"^^xsd:anyURI ;
    dcat:theme legcons:Item .

F2021L00308:93 a legcons:Item,
        owl:Class,
        dcat:Resource ;
    rdfs:label "Item - I93 5 7  Areas where post mortem inspections are carried out"@en-AU ;
    dct:isPartOf F2021L00308:91 ;
    dct:isReferencedBy F2021L00308: ;
    rdfs:comment "5 7  Areas where post mortem inspections are carried out - Abrievated Graph Key: I93"@en-AU ;
    skos:definition "5 7  Areas where post mortem inspections are carried out"@en-AU ;
    skos:narrower F2021L00308:91 ;
    skos:prefLabel "Item I93"@en-AU ;
    dcat:accessURL <https://www.legislation.gov.au/F2021L00308/2023-08-04/2023-08-04/text/original/epub/OEBPS/document_1/document_1.html#_Toc143604802> ;
    dcat:landingPage "https://www.legislation.gov.au/F2021L00308/2023-08-04/2023-08-04/text/original/epub/OEBPS/document_1/document_1.html#_Toc143604802"^^xsd:anyURI ;
    dcat:theme legcons:Item .

F2021L00308:94 a legcons:Item,
        owl:Class,
        dcat:Resource ;
    rdfs:label "Item - I94 5 8  Compliance with decisions and dispositions"@en-AU ;
    dct:isPartOf F2021L00308:91 ;
    dct:isReferencedBy F2021L00308: ;
    rdfs:comment "5 8  Compliance with decisions and dispositions - Abrievated Graph Key: I94"@en-AU ;
    skos:definition "5 8  Compliance with decisions and dispositions"@en-AU ;
    skos:narrower F2021L00308:91 ;
    skos:prefLabel "Item I94"@en-AU ;
    dcat:accessURL <https://www.legislation.gov.au/F2021L00308/2023-08-04/2023-08-04/text/original/epub/OEBPS/document_1/document_1.html#_Toc143604803> ;
    dcat:landingPage "https://www.legislation.gov.au/F2021L00308/2023-08-04/2023-08-04/text/original/epub/OEBPS/document_1/document_1.html#_Toc143604803"^^xsd:anyURI ;
    dcat:theme legcons:Item .

F2021L00308:95 a legcons:Subdivision,
        owl:Class,
        dcat:Resource ;
    rdfs:label "Subdivision - S95 Subdivision BOther requirements rabbits"@en-AU ;
    dct:isPartOf F2021L00308:90 ;
    dct:isReferencedBy F2021L00308: ;
    rdfs:comment "Subdivision BOther requirements rabbits - Abrievated Graph Key: S95"@en-AU ;
    skos:definition "Subdivision BOther requirements rabbits"@en-AU ;
    skos:narrower F2021L00308:90 ;
    skos:prefLabel "Subdivision S95"@en-AU ;
    dcat:accessURL <https://www.legislation.gov.au/F2021L00308/2023-08-04/2023-08-04/text/original/epub/OEBPS/document_1/document_1.html#_Toc143604804> ;
    dcat:landingPage "https://www.legislation.gov.au/F2021L00308/2023-08-04/2023-08-04/text/original/epub/OEBPS/document_1/document_1.html#_Toc143604804"^^xsd:anyURI ;
    dcat:theme legcons:Subdivision .

F2021L00308:96 a legcons:Item,
        owl:Class,
        dcat:Resource ;
    rdfs:label "Item - I96 5 9  Separation of rabbit carcases"@en-AU ;
    dct:isPartOf F2021L00308:90 ;
    dct:isReferencedBy F2021L00308: ;
    rdfs:comment "5 9  Separation of rabbit carcases - Abrievated Graph Key: I96"@en-AU ;
    skos:definition "5 9  Separation of rabbit carcases"@en-AU ;
    skos:narrower F2021L00308:90 ;
    skos:prefLabel "Item I96"@en-AU ;
    dcat:accessURL <https://www.legislation.gov.au/F2021L00308/2023-08-04/2023-08-04/text/original/epub/OEBPS/document_1/document_1.html#_Toc143604805> ;
    dcat:landingPage "https://www.legislation.gov.au/F2021L00308/2023-08-04/2023-08-04/text/original/epub/OEBPS/document_1/document_1.html#_Toc143604805"^^xsd:anyURI ;
    dcat:theme legcons:Item .

F2021L00308:97 a legcons:Subdivision,
        owl:Class,
        dcat:Resource ;
    rdfs:label "Subdivision - S97 Subdivision COther requirements ratites"@en-AU ;
    dct:isPartOf F2021L00308:90 ;
    dct:isReferencedBy F2021L00308: ;
    rdfs:comment "Subdivision COther requirements ratites - Abrievated Graph Key: S97"@en-AU ;
    skos:definition "Subdivision COther requirements ratites"@en-AU ;
    skos:narrower F2021L00308:90 ;
    skos:prefLabel "Subdivision S97"@en-AU ;
    dcat:accessURL <https://www.legislation.gov.au/F2021L00308/2023-08-04/2023-08-04/text/original/epub/OEBPS/document_1/document_1.html#_Toc143604806> ;
    dcat:landingPage "https://www.legislation.gov.au/F2021L00308/2023-08-04/2023-08-04/text/original/epub/OEBPS/document_1/document_1.html#_Toc143604806"^^xsd:anyURI ;
    dcat:theme legcons:Subdivision .

F2021L00308:98 a legcons:Item,
        owl:Class,
        dcat:Resource ;
    rdfs:label "Item - I98 5 10  Humane treatment of ratites"@en-AU ;
    dct:isPartOf F2021L00308:90 ;
    dct:isReferencedBy F2021L00308: ;
    rdfs:comment "5 10  Humane treatment of ratites - Abrievated Graph Key: I98"@en-AU ;
    skos:definition "5 10  Humane treatment of ratites"@en-AU ;
    skos:narrower F2021L00308:90 ;
    skos:prefLabel "Item I98"@en-AU ;
    dcat:accessURL <https://www.legislation.gov.au/F2021L00308/2023-08-04/2023-08-04/text/original/epub/OEBPS/document_1/document_1.html#_Toc143604807> ;
    dcat:landingPage "https://www.legislation.gov.au/F2021L00308/2023-08-04/2023-08-04/text/original/epub/OEBPS/document_1/document_1.html#_Toc143604807"^^xsd:anyURI ;
    dcat:theme legcons:Item .

F2021L00308:99 a legcons:Item,
        owl:Class,
        dcat:Resource ;
    rdfs:label "Item - I99 5 11  Ante mortem treatment of ratites"@en-AU ;
    dct:isPartOf F2021L00308:90 ;
    dct:isReferencedBy F2021L00308: ;
    rdfs:comment "5 11  Ante mortem treatment of ratites - Abrievated Graph Key: I99"@en-AU ;
    skos:definition "5 11  Ante mortem treatment of ratites"@en-AU ;
    skos:narrower F2021L00308:90 ;
    skos:prefLabel "Item I99"@en-AU ;
    dcat:accessURL <https://www.legislation.gov.au/F2021L00308/2023-08-04/2023-08-04/text/original/epub/OEBPS/document_1/document_1.html#_Toc143604808> ;
    dcat:landingPage "https://www.legislation.gov.au/F2021L00308/2023-08-04/2023-08-04/text/original/epub/OEBPS/document_1/document_1.html#_Toc143604808"^^xsd:anyURI ;
    dcat:theme legcons:Item .

F2021L00308:148 a legcons:Division,
        owl:Class,
        dcat:Resource ;
    rdfs:label "Division - D148 Division 2 Variations required by Secretary"@en-AU ;
    dct:hasPart F2021L00308:149 ;
    dct:isPartOf F2021L00308:80 ;
    dct:isReferencedBy F2021L00308: ;
    rdfs:comment "Division 2 Variations required by Secretary - Abrievated Graph Key: D148"@en-AU ;
    skos:broader F2021L00308:149 ;
    skos:definition "Division 2 Variations required by Secretary"@en-AU ;
    skos:narrower F2021L00308:80 ;
    skos:prefLabel "Division D148"@en-AU ;
    dcat:accessURL <https://www.legislation.gov.au/F2021L00308/2023-08-04/2023-08-04/text/original/epub/OEBPS/document_1/document_1.html#_Toc143604857> ;
    dcat:landingPage "https://www.legislation.gov.au/F2021L00308/2023-08-04/2023-08-04/text/original/epub/OEBPS/document_1/document_1.html#_Toc143604857"^^xsd:anyURI ;
    dcat:theme legcons:Division .

F2021L00308:155 a legcons:Part,
        owl:Class,
        dcat:Resource ;
    rdfs:label "Part - P155 Part 1 Issue of export permit"@en-AU ;
    dct:hasPart F2021L00308:156 ;
    dct:isPartOf F2021L00308:154 ;
    dct:isReferencedBy F2021L00308: ;
    rdfs:comment "Part 1 Issue of export permit - Abrievated Graph Key: P155"@en-AU ;
    skos:broader F2021L00308:156 ;
    skos:definition "Part 1 Issue of export permit"@en-AU ;
    skos:narrower F2021L00308:154 ;
    skos:prefLabel "Part P155"@en-AU ;
    dcat:accessURL <https://www.legislation.gov.au/F2021L00308/2023-08-04/2023-08-04/text/original/epub/OEBPS/document_1/document_1.html#_Toc143604864> ;
    dcat:landingPage "https://www.legislation.gov.au/F2021L00308/2023-08-04/2023-08-04/text/original/epub/OEBPS/document_1/document_1.html#_Toc143604864"^^xsd:anyURI ;
    dcat:theme legcons:Part .

F2021L00308:214 a legcons:Division,
        owl:Class,
        dcat:Resource ;
    rdfs:label "Division - D214 Division 1 General"@en-AU ;
    dct:hasPart F2021L00308:215 ;
    dct:isPartOf F2021L00308:213 ;
    dct:isReferencedBy F2021L00308: ;
    rdfs:comment "Division 1 General - Abrievated Graph Key: D214"@en-AU ;
    skos:broader F2021L00308:215 ;
    skos:definition "Division 1 General"@en-AU ;
    skos:narrower F2021L00308:213 ;
    skos:prefLabel "Division D214"@en-AU ;
    dcat:accessURL <https://www.legislation.gov.au/F2021L00308/2023-08-04/2023-08-04/text/original/epub/OEBPS/document_1/document_1.html#_Toc143604923> ;
    dcat:landingPage "https://www.legislation.gov.au/F2021L00308/2023-08-04/2023-08-04/text/original/epub/OEBPS/document_1/document_1.html#_Toc143604923"^^xsd:anyURI ;
    dcat:theme legcons:Division .

F2021L00308:233 a legcons:Part,
        owl:Class,
        dcat:Resource ;
    rdfs:label "Part - P233 Part 2 Assessments"@en-AU ;
    dct:hasPart F2021L00308:234 ;
    dct:isPartOf F2021L00308:212 ;
    dct:isReferencedBy F2021L00308: ;
    rdfs:comment "Part 2 Assessments - Abrievated Graph Key: P233"@en-AU ;
    skos:broader F2021L00308:234 ;
    skos:definition "Part 2 Assessments"@en-AU ;
    skos:narrower F2021L00308:212 ;
    skos:prefLabel "Part P233"@en-AU ;
    dcat:accessURL <https://www.legislation.gov.au/F2021L00308/2023-08-04/2023-08-04/text/original/epub/OEBPS/document_1/document_1.html#_Toc143604942> ;
    dcat:landingPage "https://www.legislation.gov.au/F2021L00308/2023-08-04/2023-08-04/text/original/epub/OEBPS/document_1/document_1.html#_Toc143604942"^^xsd:anyURI ;
    dcat:theme legcons:Part .

F2021L00308:235 a legcons:Part,
        owl:Class,
        dcat:Resource ;
    rdfs:label "Part - P235 Part 3 Powers of the Secretary"@en-AU ;
    dct:hasPart F2021L00308:236 ;
    dct:isPartOf F2021L00308:212 ;
    dct:isReferencedBy F2021L00308: ;
    rdfs:comment "Part 3 Powers of the Secretary - Abrievated Graph Key: P235"@en-AU ;
    skos:broader F2021L00308:236 ;
    skos:definition "Part 3 Powers of the Secretary"@en-AU ;
    skos:narrower F2021L00308:212 ;
    skos:prefLabel "Part P235"@en-AU ;
    dcat:accessURL <https://www.legislation.gov.au/F2021L00308/2023-08-04/2023-08-04/text/original/epub/OEBPS/document_1/document_1.html#_Toc143604944> ;
    dcat:landingPage "https://www.legislation.gov.au/F2021L00308/2023-08-04/2023-08-04/text/original/epub/OEBPS/document_1/document_1.html#_Toc143604944"^^xsd:anyURI ;
    dcat:theme legcons:Part .

F2021L00308:238 a legcons:Division,
        owl:Class,
        dcat:Resource ;
    rdfs:label "Division - D238 Division 1 Third party authorised officers"@en-AU ;
    dct:hasPart F2021L00308:239 ;
    dct:isPartOf F2021L00308:237 ;
    dct:isReferencedBy F2021L00308: ;
    rdfs:comment "Division 1 Third party authorised officers - Abrievated Graph Key: D238"@en-AU ;
    skos:broader F2021L00308:239 ;
    skos:definition "Division 1 Third party authorised officers"@en-AU ;
    skos:narrower F2021L00308:237 ;
    skos:prefLabel "Division D238"@en-AU ;
    dcat:accessURL <https://www.legislation.gov.au/F2021L00308/2023-08-04/2023-08-04/text/original/epub/OEBPS/document_1/document_1.html#_Toc143604947> ;
    dcat:landingPage "https://www.legislation.gov.au/F2021L00308/2023-08-04/2023-08-04/text/original/epub/OEBPS/document_1/document_1.html#_Toc143604947"^^xsd:anyURI ;
    dcat:theme legcons:Division .

F2021L00308:257 a legcons:Division,
        owl:Class,
        dcat:Resource ;
    rdfs:label "Division - D257 Division 3 Directions to deal with non compliance with the Act etc"@en-AU ;
    dct:hasPart F2021L00308:258 ;
    dct:isPartOf F2021L00308:237 ;
    dct:isReferencedBy F2021L00308: ;
    rdfs:comment "Division 3 Directions to deal with non compliance with the Act etc - Abrievated Graph Key: D257"@en-AU ;
    skos:broader F2021L00308:258 ;
    skos:definition "Division 3 Directions to deal with non compliance with the Act etc"@en-AU ;
    skos:narrower F2021L00308:237 ;
    skos:prefLabel "Division D257"@en-AU ;
    dcat:accessURL <https://www.legislation.gov.au/F2021L00308/2023-08-04/2023-08-04/text/original/epub/OEBPS/document_1/document_1.html#_Toc143604966> ;
    dcat:landingPage "https://www.legislation.gov.au/F2021L00308/2023-08-04/2023-08-04/text/original/epub/OEBPS/document_1/document_1.html#_Toc143604966"^^xsd:anyURI ;
    dcat:theme legcons:Division .

F2021L00308:259 a legcons:Division,
        owl:Class,
        dcat:Resource ;
    rdfs:label "Division - D259 Division 4 Miscellaneous"@en-AU ;
    dct:hasPart F2021L00308:260 ;
    dct:isPartOf F2021L00308:237 ;
    dct:isReferencedBy F2021L00308: ;
    rdfs:comment "Division 4 Miscellaneous - Abrievated Graph Key: D259"@en-AU ;
    skos:broader F2021L00308:260 ;
    skos:definition "Division 4 Miscellaneous"@en-AU ;
    skos:narrower F2021L00308:237 ;
    skos:prefLabel "Division D259"@en-AU ;
    dcat:accessURL <https://www.legislation.gov.au/F2021L00308/2023-08-04/2023-08-04/text/original/epub/OEBPS/document_1/document_1.html#_Toc143604968> ;
    dcat:landingPage "https://www.legislation.gov.au/F2021L00308/2023-08-04/2023-08-04/text/original/epub/OEBPS/document_1/document_1.html#_Toc143604968"^^xsd:anyURI ;
    dcat:theme legcons:Division .

F2021L00308:261 a legcons:Chapter,
        owl:Class,
        dcat:Resource ;
    rdfs:label "Chapter - C261 Chapter 10 Compliance and enforcement"@en-AU ;
    dct:hasPart F2021L00308:262,
        F2021L00308:263 ;
    dct:isReferencedBy F2021L00308: ;
    rdfs:comment "Chapter 10 Compliance and enforcement - Abrievated Graph Key: C261"@en-AU ;
    skos:broader F2021L00308:262,
        F2021L00308:263 ;
    skos:definition "Chapter 10 Compliance and enforcement"@en-AU ;
    skos:prefLabel "Chapter C261"@en-AU ;
    dcat:accessURL <https://www.legislation.gov.au/F2021L00308/2023-08-04/2023-08-04/text/original/epub/OEBPS/document_1/document_1.html#_Toc143604970> ;
    dcat:landingPage "https://www.legislation.gov.au/F2021L00308/2023-08-04/2023-08-04/text/original/epub/OEBPS/document_1/document_1.html#_Toc143604970"^^xsd:anyURI ;
    dcat:theme legcons:Chapter .

F2021L00308:265 a legcons:Part,
        owl:Class,
        dcat:Resource ;
    rdfs:label "Part - P265 Part 1 Review of decisions"@en-AU ;
    dct:hasPart F2021L00308:266 ;
    dct:isPartOf F2021L00308:264 ;
    dct:isReferencedBy F2021L00308: ;
    rdfs:comment "Part 1 Review of decisions - Abrievated Graph Key: P265"@en-AU ;
    skos:broader F2021L00308:266 ;
    skos:definition "Part 1 Review of decisions"@en-AU ;
    skos:narrower F2021L00308:264 ;
    skos:prefLabel "Part P265"@en-AU ;
    dcat:accessURL <https://www.legislation.gov.au/F2021L00308/2023-08-04/2023-08-04/text/original/epub/OEBPS/document_1/document_1.html#_Toc143604974> ;
    dcat:landingPage "https://www.legislation.gov.au/F2021L00308/2023-08-04/2023-08-04/text/original/epub/OEBPS/document_1/document_1.html#_Toc143604974"^^xsd:anyURI ;
    dcat:theme legcons:Part .

F2021L00308:278 a legcons:Part,
        owl:Class,
        dcat:Resource ;
    rdfs:label "Part - P278 Part 3 Samples"@en-AU ;
    dct:hasPart F2021L00308:279 ;
    dct:isPartOf F2021L00308:264 ;
    dct:isReferencedBy F2021L00308: ;
    rdfs:comment "Part 3 Samples - Abrievated Graph Key: P278"@en-AU ;
    skos:broader F2021L00308:279 ;
    skos:definition "Part 3 Samples"@en-AU ;
    skos:narrower F2021L00308:264 ;
    skos:prefLabel "Part P278"@en-AU ;
    dcat:accessURL <https://www.legislation.gov.au/F2021L00308/2023-08-04/2023-08-04/text/original/epub/OEBPS/document_1/document_1.html#_Toc143604987> ;
    dcat:landingPage "https://www.legislation.gov.au/F2021L00308/2023-08-04/2023-08-04/text/original/epub/OEBPS/document_1/document_1.html#_Toc143604987"^^xsd:anyURI ;
    dcat:theme legcons:Part .

F2021L00308:283 a legcons:Part,
        owl:Class,
        dcat:Resource ;
    rdfs:label "Part - P283 Part 5 Relevant Commonwealth liabilities"@en-AU ;
    dct:hasPart F2021L00308:284 ;
    dct:isPartOf F2021L00308:264 ;
    dct:isReferencedBy F2021L00308: ;
    rdfs:comment "Part 5 Relevant Commonwealth liabilities - Abrievated Graph Key: P283"@en-AU ;
    skos:broader F2021L00308:284 ;
    skos:definition "Part 5 Relevant Commonwealth liabilities"@en-AU ;
    skos:narrower F2021L00308:264 ;
    skos:prefLabel "Part P283"@en-AU ;
    dcat:accessURL <https://www.legislation.gov.au/F2021L00308/2023-08-04/2023-08-04/text/original/epub/OEBPS/document_1/document_1.html#_Toc143604992> ;
    dcat:landingPage "https://www.legislation.gov.au/F2021L00308/2023-08-04/2023-08-04/text/original/epub/OEBPS/document_1/document_1.html#_Toc143604992"^^xsd:anyURI ;
    dcat:theme legcons:Part .

F2021L00308:286 a legcons:Part,
        owl:Class,
        dcat:Resource ;
    rdfs:label "Part - P286 Part 1 Preliminary"@en-AU ;
    dct:hasPart F2021L00308:287 ;
    dct:isPartOf F2021L00308:285 ;
    dct:isReferencedBy F2021L00308: ;
    rdfs:comment "Part 1 Preliminary - Abrievated Graph Key: P286"@en-AU ;
    skos:broader F2021L00308:287 ;
    skos:definition "Part 1 Preliminary"@en-AU ;
    skos:narrower F2021L00308:285 ;
    skos:prefLabel "Part P286"@en-AU ;
    dcat:accessURL <https://www.legislation.gov.au/F2021L00308/2023-08-04/2023-08-04/text/original/epub/OEBPS/document_1/document_1.html#_Toc143604995> ;
    dcat:landingPage "https://www.legislation.gov.au/F2021L00308/2023-08-04/2023-08-04/text/original/epub/OEBPS/document_1/document_1.html#_Toc143604995"^^xsd:anyURI ;
    dcat:theme legcons:Part .

F2021L00308:296 a legcons:Part,
        owl:Class,
        dcat:Resource ;
    rdfs:label "Part - P296 Part 3 Powers and officials"@en-AU ;
    dct:hasPart F2021L00308:297 ;
    dct:isPartOf F2021L00308:285 ;
    dct:isReferencedBy F2021L00308: ;
    rdfs:comment "Part 3 Powers and officials - Abrievated Graph Key: P296"@en-AU ;
    skos:broader F2021L00308:297 ;
    skos:definition "Part 3 Powers and officials"@en-AU ;
    skos:narrower F2021L00308:285 ;
    skos:prefLabel "Part P296"@en-AU ;
    dcat:accessURL <https://www.legislation.gov.au/F2021L00308/2023-08-04/2023-08-04/text/original/epub/OEBPS/document_1/document_1.html#_Toc143605005> ;
    dcat:landingPage "https://www.legislation.gov.au/F2021L00308/2023-08-04/2023-08-04/text/original/epub/OEBPS/document_1/document_1.html#_Toc143605005"^^xsd:anyURI ;
    dcat:theme legcons:Part .

F2021L00308:299 a legcons:Part,
        owl:Class,
        dcat:Resource ;
    rdfs:label "Part - P299 Part 1 Rabbit carcases or carcase parts"@en-AU ;
    dct:hasPart F2021L00308:300 ;
    dct:isPartOf F2021L00308:298 ;
    dct:isReferencedBy F2021L00308: ;
    rdfs:comment "Part 1 Rabbit carcases or carcase parts - Abrievated Graph Key: P299"@en-AU ;
    skos:broader F2021L00308:300 ;
    skos:definition "Part 1 Rabbit carcases or carcase parts"@en-AU ;
    skos:narrower F2021L00308:298 ;
    skos:prefLabel "Part P299"@en-AU ;
    dcat:accessURL <https://www.legislation.gov.au/F2021L00308/2023-08-04/2023-08-04/text/original/epub/OEBPS/document_1/document_1.html#_Toc143605008> ;
    dcat:landingPage "https://www.legislation.gov.au/F2021L00308/2023-08-04/2023-08-04/text/original/epub/OEBPS/document_1/document_1.html#_Toc143605008"^^xsd:anyURI ;
    dcat:theme legcons:Part .

F2021L00308:301 a legcons:Part,
        owl:Class,
        dcat:Resource ;
    rdfs:label "Part - P301 Part 2 Ratite carcases or carcase parts"@en-AU ;
    dct:hasPart F2021L00308:302 ;
    dct:isPartOf F2021L00308:298 ;
    dct:isReferencedBy F2021L00308: ;
    rdfs:comment "Part 2 Ratite carcases or carcase parts - Abrievated Graph Key: P301"@en-AU ;
    skos:broader F2021L00308:302 ;
    skos:definition "Part 2 Ratite carcases or carcase parts"@en-AU ;
    skos:narrower F2021L00308:298 ;
    skos:prefLabel "Part P301"@en-AU ;
    dcat:accessURL <https://www.legislation.gov.au/F2021L00308/2023-08-04/2023-08-04/text/original/epub/OEBPS/document_1/document_1.html#_Toc143605010> ;
    dcat:landingPage "https://www.legislation.gov.au/F2021L00308/2023-08-04/2023-08-04/text/original/epub/OEBPS/document_1/document_1.html#_Toc143605010"^^xsd:anyURI ;
    dcat:theme legcons:Part .

F2021L00308:58 a legcons:Part,
        owl:Class,
        dcat:Resource ;
    rdfs:label "Part - P58 Part 4 Variation of registration"@en-AU ;
    dct:hasPart F2021L00308:59 ;
    dct:isPartOf F2021L00308:35 ;
    dct:isReferencedBy F2021L00308: ;
    rdfs:comment "Part 4 Variation of registration - Abrievated Graph Key: P58"@en-AU ;
    skos:broader F2021L00308:59 ;
    skos:definition "Part 4 Variation of registration"@en-AU ;
    skos:narrower F2021L00308:35 ;
    skos:prefLabel "Part P58"@en-AU ;
    dcat:accessURL <https://www.legislation.gov.au/F2021L00308/2023-08-04/2023-08-04/text/original/epub/OEBPS/document_1/document_1.html#_Toc143604767> ;
    dcat:landingPage "https://www.legislation.gov.au/F2021L00308/2023-08-04/2023-08-04/text/original/epub/OEBPS/document_1/document_1.html#_Toc143604767"^^xsd:anyURI ;
    dcat:theme legcons:Part .

F2021L00308:85 a legcons:Division,
        owl:Class,
        dcat:Resource ;
    rdfs:label "Division - D85 Division 1 Purpose of this Part"@en-AU ;
    dct:hasPart F2021L00308:86 ;
    dct:isPartOf F2021L00308:84 ;
    dct:isReferencedBy F2021L00308: ;
    rdfs:comment "Division 1 Purpose of this Part - Abrievated Graph Key: D85"@en-AU ;
    skos:broader F2021L00308:86 ;
    skos:definition "Division 1 Purpose of this Part"@en-AU ;
    skos:narrower F2021L00308:84 ;
    skos:prefLabel "Division D85"@en-AU ;
    dcat:accessURL <https://www.legislation.gov.au/F2021L00308/2023-08-04/2023-08-04/text/original/epub/OEBPS/document_1/document_1.html#_Toc143604794> ;
    dcat:landingPage "https://www.legislation.gov.au/F2021L00308/2023-08-04/2023-08-04/text/original/epub/OEBPS/document_1/document_1.html#_Toc143604794"^^xsd:anyURI ;
    dcat:theme legcons:Division .

F2021L00308:14 a legcons:Chapter,
        owl:Class,
        dcat:Resource ;
    rdfs:label "Chapter - C14 Chapter 2 Exporting goods"@en-AU ;
    dct:hasPart F2021L00308:15,
        F2021L00308:22,
        F2021L00308:29 ;
    dct:isReferencedBy F2021L00308: ;
    rdfs:comment "Chapter 2 Exporting goods - Abrievated Graph Key: C14"@en-AU ;
    skos:broader F2021L00308:15,
        F2021L00308:22,
        F2021L00308:29 ;
    skos:definition "Chapter 2 Exporting goods"@en-AU ;
    skos:prefLabel "Chapter C14"@en-AU ;
    dcat:accessURL <https://www.legislation.gov.au/F2021L00308/2023-08-04/2023-08-04/text/original/epub/OEBPS/document_1/document_1.html#_Toc143604723> ;
    dcat:landingPage "https://www.legislation.gov.au/F2021L00308/2023-08-04/2023-08-04/text/original/epub/OEBPS/document_1/document_1.html#_Toc143604723"^^xsd:anyURI ;
    dcat:theme legcons:Chapter .

F2021L00308:145 a legcons:Division,
        owl:Class,
        dcat:Resource ;
    rdfs:label "Division - D145 Division 1 Variations by holder"@en-AU ;
    dct:hasPart F2021L00308:146,
        F2021L00308:147 ;
    dct:isPartOf F2021L00308:80 ;
    dct:isReferencedBy F2021L00308: ;
    rdfs:comment "Division 1 Variations by holder - Abrievated Graph Key: D145"@en-AU ;
    skos:broader F2021L00308:146,
        F2021L00308:147 ;
    skos:definition "Division 1 Variations by holder"@en-AU ;
    skos:narrower F2021L00308:80 ;
    skos:prefLabel "Division D145"@en-AU ;
    dcat:accessURL <https://www.legislation.gov.au/F2021L00308/2023-08-04/2023-08-04/text/original/epub/OEBPS/document_1/document_1.html#_Toc143604854> ;
    dcat:landingPage "https://www.legislation.gov.au/F2021L00308/2023-08-04/2023-08-04/text/original/epub/OEBPS/document_1/document_1.html#_Toc143604854"^^xsd:anyURI ;
    dcat:theme legcons:Division .

F2021L00308:15 a legcons:Part,
        owl:Class,
        dcat:Resource ;
    rdfs:label "Part - P15 Part 1 Goods"@en-AU ;
    dct:hasPart F2021L00308:16,
        F2021L00308:19 ;
    dct:isPartOf F2021L00308:14 ;
    dct:isReferencedBy F2021L00308: ;
    rdfs:comment "Part 1 Goods - Abrievated Graph Key: P15"@en-AU ;
    skos:broader F2021L00308:16,
        F2021L00308:19 ;
    skos:definition "Part 1 Goods"@en-AU ;
    skos:narrower F2021L00308:14 ;
    skos:prefLabel "Part P15"@en-AU ;
    dcat:accessURL <https://www.legislation.gov.au/F2021L00308/2023-08-04/2023-08-04/text/original/epub/OEBPS/document_1/document_1.html#_Toc143604724> ;
    dcat:landingPage "https://www.legislation.gov.au/F2021L00308/2023-08-04/2023-08-04/text/original/epub/OEBPS/document_1/document_1.html#_Toc143604724"^^xsd:anyURI ;
    dcat:theme legcons:Part .

F2021L00308:154 a legcons:Chapter,
        owl:Class,
        dcat:Resource ;
    rdfs:label "Chapter - C154 Chapter 7 Export permits"@en-AU ;
    dct:hasPart F2021L00308:155,
        F2021L00308:157,
        F2021L00308:161 ;
    dct:isReferencedBy F2021L00308: ;
    rdfs:comment "Chapter 7 Export permits - Abrievated Graph Key: C154"@en-AU ;
    skos:broader F2021L00308:155,
        F2021L00308:157,
        F2021L00308:161 ;
    skos:definition "Chapter 7 Export permits"@en-AU ;
    skos:prefLabel "Chapter C154"@en-AU ;
    dcat:accessURL <https://www.legislation.gov.au/F2021L00308/2023-08-04/2023-08-04/text/original/epub/OEBPS/document_1/document_1.html#_Toc143604863> ;
    dcat:landingPage "https://www.legislation.gov.au/F2021L00308/2023-08-04/2023-08-04/text/original/epub/OEBPS/document_1/document_1.html#_Toc143604863"^^xsd:anyURI ;
    dcat:theme legcons:Chapter .

F2021L00308:16 a legcons:Division,
        owl:Class,
        dcat:Resource ;
    rdfs:label "Division - D16 Division 1 Prescribed goods"@en-AU ;
    dct:hasPart F2021L00308:17,
        F2021L00308:18 ;
    dct:isPartOf F2021L00308:15 ;
    dct:isReferencedBy F2021L00308: ;
    rdfs:comment "Division 1 Prescribed goods - Abrievated Graph Key: D16"@en-AU ;
    skos:broader F2021L00308:17,
        F2021L00308:18 ;
    skos:definition "Division 1 Prescribed goods"@en-AU ;
    skos:narrower F2021L00308:15 ;
    skos:prefLabel "Division D16"@en-AU ;
    dcat:accessURL <https://www.legislation.gov.au/F2021L00308/2023-08-04/2023-08-04/text/original/epub/OEBPS/document_1/document_1.html#_Toc143604725> ;
    dcat:landingPage "https://www.legislation.gov.au/F2021L00308/2023-08-04/2023-08-04/text/original/epub/OEBPS/document_1/document_1.html#_Toc143604725"^^xsd:anyURI ;
    dcat:theme legcons:Division .

F2021L00308:166 a legcons:Chapter,
        owl:Class,
        dcat:Resource ;
    rdfs:label "Chapter - C166 Chapter 8 Other matters relating to export"@en-AU ;
    dct:hasPart F2021L00308:167,
        F2021L00308:172,
        F2021L00308:176 ;
    dct:isReferencedBy F2021L00308: ;
    rdfs:comment "Chapter 8 Other matters relating to export - Abrievated Graph Key: C166"@en-AU ;
    skos:broader F2021L00308:167,
        F2021L00308:172,
        F2021L00308:176 ;
    skos:definition "Chapter 8 Other matters relating to export"@en-AU ;
    skos:prefLabel "Chapter C166"@en-AU ;
    dcat:accessURL <https://www.legislation.gov.au/F2021L00308/2023-08-04/2023-08-04/text/original/epub/OEBPS/document_1/document_1.html#_Toc143604875> ;
    dcat:landingPage "https://www.legislation.gov.au/F2021L00308/2023-08-04/2023-08-04/text/original/epub/OEBPS/document_1/document_1.html#_Toc143604875"^^xsd:anyURI ;
    dcat:theme legcons:Chapter .

F2021L00308:19 a legcons:Division,
        owl:Class,
        dcat:Resource ;
    rdfs:label "Division - D19 Division 2 Prohibited export and prescribed export conditions"@en-AU ;
    dct:hasPart F2021L00308:20,
        F2021L00308:21 ;
    dct:isPartOf F2021L00308:15 ;
    dct:isReferencedBy F2021L00308: ;
    rdfs:comment "Division 2 Prohibited export and prescribed export conditions - Abrievated Graph Key: D19"@en-AU ;
    skos:broader F2021L00308:20,
        F2021L00308:21 ;
    skos:definition "Division 2 Prohibited export and prescribed export conditions"@en-AU ;
    skos:narrower F2021L00308:15 ;
    skos:prefLabel "Division D19"@en-AU ;
    dcat:accessURL <https://www.legislation.gov.au/F2021L00308/2023-08-04/2023-08-04/text/original/epub/OEBPS/document_1/document_1.html#_Toc143604728> ;
    dcat:landingPage "https://www.legislation.gov.au/F2021L00308/2023-08-04/2023-08-04/text/original/epub/OEBPS/document_1/document_1.html#_Toc143604728"^^xsd:anyURI ;
    dcat:theme legcons:Division .

F2021L00308:280 a legcons:Part,
        owl:Class,
        dcat:Resource ;
    rdfs:label "Part - P280 Part 4 Damaged or destroyed rabbit meat ratite meat rabbit meat products or ratite meat products"@en-AU ;
    dct:hasPart F2021L00308:281,
        F2021L00308:282 ;
    dct:isPartOf F2021L00308:264 ;
    dct:isReferencedBy F2021L00308: ;
    rdfs:comment "Part 4 Damaged or destroyed rabbit meat ratite meat rabbit meat products or ratite meat products - Abrievated Graph Key: P280"@en-AU ;
    skos:broader F2021L00308:281,
        F2021L00308:282 ;
    skos:definition "Part 4 Damaged or destroyed rabbit meat ratite meat rabbit meat products or ratite meat products"@en-AU ;
    skos:narrower F2021L00308:264 ;
    skos:prefLabel "Part P280"@en-AU ;
    dcat:accessURL <https://www.legislation.gov.au/F2021L00308/2023-08-04/2023-08-04/text/original/epub/OEBPS/document_1/document_1.html#_Toc143604989> ;
    dcat:landingPage "https://www.legislation.gov.au/F2021L00308/2023-08-04/2023-08-04/text/original/epub/OEBPS/document_1/document_1.html#_Toc143604989"^^xsd:anyURI ;
    dcat:theme legcons:Part .

F2021L00308:285 a legcons:Chapter,
        owl:Class,
        dcat:Resource ;
    rdfs:label "Chapter - C285 Chapter 12 Transitional provisions"@en-AU ;
    dct:hasPart F2021L00308:286,
        F2021L00308:288,
        F2021L00308:296 ;
    dct:isReferencedBy F2021L00308: ;
    rdfs:comment "Chapter 12 Transitional provisions - Abrievated Graph Key: C285"@en-AU ;
    skos:broader F2021L00308:286,
        F2021L00308:288,
        F2021L00308:296 ;
    skos:definition "Chapter 12 Transitional provisions"@en-AU ;
    skos:prefLabel "Chapter C285"@en-AU ;
    dcat:accessURL <https://www.legislation.gov.au/F2021L00308/2023-08-04/2023-08-04/text/original/epub/OEBPS/document_1/document_1.html#_Toc143604994> ;
    dcat:landingPage "https://www.legislation.gov.au/F2021L00308/2023-08-04/2023-08-04/text/original/epub/OEBPS/document_1/document_1.html#_Toc143604994"^^xsd:anyURI ;
    dcat:theme legcons:Chapter .

F2021L00308:288 a legcons:Part,
        owl:Class,
        dcat:Resource ;
    rdfs:label "Part - P288 Part 2 Other matters relating to export"@en-AU ;
    dct:hasPart F2021L00308:289,
        F2021L00308:293 ;
    dct:isPartOf F2021L00308:285 ;
    dct:isReferencedBy F2021L00308: ;
    rdfs:comment "Part 2 Other matters relating to export - Abrievated Graph Key: P288"@en-AU ;
    skos:broader F2021L00308:289,
        F2021L00308:293 ;
    skos:definition "Part 2 Other matters relating to export"@en-AU ;
    skos:narrower F2021L00308:285 ;
    skos:prefLabel "Part P288"@en-AU ;
    dcat:accessURL <https://www.legislation.gov.au/F2021L00308/2023-08-04/2023-08-04/text/original/epub/OEBPS/document_1/document_1.html#_Toc143604997> ;
    dcat:landingPage "https://www.legislation.gov.au/F2021L00308/2023-08-04/2023-08-04/text/original/epub/OEBPS/document_1/document_1.html#_Toc143604997"^^xsd:anyURI ;
    dcat:theme legcons:Part .

F2021L00308:293 a legcons:Division,
        owl:Class,
        dcat:Resource ;
    rdfs:label "Division - D293 Division 2 Official marking devices"@en-AU ;
    dct:hasPart F2021L00308:294,
        F2021L00308:295 ;
    dct:isPartOf F2021L00308:288 ;
    dct:isReferencedBy F2021L00308: ;
    rdfs:comment "Division 2 Official marking devices - Abrievated Graph Key: D293"@en-AU ;
    skos:broader F2021L00308:294,
        F2021L00308:295 ;
    skos:definition "Division 2 Official marking devices"@en-AU ;
    skos:narrower F2021L00308:288 ;
    skos:prefLabel "Division D293"@en-AU ;
    dcat:accessURL <https://www.legislation.gov.au/F2021L00308/2023-08-04/2023-08-04/text/original/epub/OEBPS/document_1/document_1.html#_Toc143605002> ;
    dcat:landingPage "https://www.legislation.gov.au/F2021L00308/2023-08-04/2023-08-04/text/original/epub/OEBPS/document_1/document_1.html#_Toc143605002"^^xsd:anyURI ;
    dcat:theme legcons:Division .

F2021L00308:298 a legcons:Schedule,
        owl:Class,
        dcat:Resource ;
    rdfs:label "Schedule - S298 Schedule 1 Post mortem dispositions and related actions"@en-AU ;
    dct:hasPart F2021L00308:299,
        F2021L00308:301,
        F2021L00308:303 ;
    dct:isReferencedBy F2021L00308: ;
    rdfs:comment "Schedule 1 Post mortem dispositions and related actions - Abrievated Graph Key: S298"@en-AU ;
    skos:broader F2021L00308:299,
        F2021L00308:301,
        F2021L00308:303 ;
    skos:definition "Schedule 1 Post mortem dispositions and related actions"@en-AU ;
    skos:prefLabel "Schedule S298"@en-AU ;
    dcat:accessURL <https://www.legislation.gov.au/F2021L00308/2023-08-04/2023-08-04/text/original/epub/OEBPS/document_1/document_1.html#_Toc143605007> ;
    dcat:landingPage "https://www.legislation.gov.au/F2021L00308/2023-08-04/2023-08-04/text/original/epub/OEBPS/document_1/document_1.html#_Toc143605007"^^xsd:anyURI ;
    dcat:theme legcons:Schedule .

F2021L00308:55 a legcons:Part,
        owl:Class,
        dcat:Resource ;
    rdfs:label "Part - P55 Part 3 Renewal of registration"@en-AU ;
    dct:hasPart F2021L00308:56,
        F2021L00308:57 ;
    dct:isPartOf F2021L00308:35 ;
    dct:isReferencedBy F2021L00308: ;
    rdfs:comment "Part 3 Renewal of registration - Abrievated Graph Key: P55"@en-AU ;
    skos:broader F2021L00308:56,
        F2021L00308:57 ;
    skos:definition "Part 3 Renewal of registration"@en-AU ;
    skos:narrower F2021L00308:35 ;
    skos:prefLabel "Part P55"@en-AU ;
    dcat:accessURL <https://www.legislation.gov.au/F2021L00308/2023-08-04/2023-08-04/text/original/epub/OEBPS/document_1/document_1.html#_Toc143604764> ;
    dcat:landingPage "https://www.legislation.gov.au/F2021L00308/2023-08-04/2023-08-04/text/original/epub/OEBPS/document_1/document_1.html#_Toc143604764"^^xsd:anyURI ;
    dcat:theme legcons:Part .

F2021L00308:64 a legcons:Part,
        owl:Class,
        dcat:Resource ;
    rdfs:label "Part - P64 Part 6 Meat inspection services"@en-AU ;
    dct:hasPart F2021L00308:65,
        F2021L00308:74 ;
    dct:isPartOf F2021L00308:35 ;
    dct:isReferencedBy F2021L00308: ;
    rdfs:comment "Part 6 Meat inspection services - Abrievated Graph Key: P64"@en-AU ;
    skos:broader F2021L00308:65,
        F2021L00308:74 ;
    skos:definition "Part 6 Meat inspection services"@en-AU ;
    skos:narrower F2021L00308:35 ;
    skos:prefLabel "Part P64"@en-AU ;
    dcat:accessURL <https://www.legislation.gov.au/F2021L00308/2023-08-04/2023-08-04/text/original/epub/OEBPS/document_1/document_1.html#_Toc143604773> ;
    dcat:landingPage "https://www.legislation.gov.au/F2021L00308/2023-08-04/2023-08-04/text/original/epub/OEBPS/document_1/document_1.html#_Toc143604773"^^xsd:anyURI ;
    dcat:theme legcons:Part .

F2021L00308:81 a legcons:Part,
        owl:Class,
        dcat:Resource ;
    rdfs:label "Part - P81 Part 1 Requirements for approval"@en-AU ;
    dct:hasPart F2021L00308:82,
        F2021L00308:83 ;
    dct:isPartOf F2021L00308:80 ;
    dct:isReferencedBy F2021L00308: ;
    rdfs:comment "Part 1 Requirements for approval - Abrievated Graph Key: P81"@en-AU ;
    skos:broader F2021L00308:82,
        F2021L00308:83 ;
    skos:definition "Part 1 Requirements for approval"@en-AU ;
    skos:narrower F2021L00308:80 ;
    skos:prefLabel "Part P81"@en-AU ;
    dcat:accessURL <https://www.legislation.gov.au/F2021L00308/2023-08-04/2023-08-04/text/original/epub/OEBPS/document_1/document_1.html#_Toc143604790> ;
    dcat:landingPage "https://www.legislation.gov.au/F2021L00308/2023-08-04/2023-08-04/text/original/epub/OEBPS/document_1/document_1.html#_Toc143604790"^^xsd:anyURI ;
    dcat:theme legcons:Part .

F2021L00308:87 a legcons:Division,
        owl:Class,
        dcat:Resource ;
    rdfs:label "Division - D87 Division 2 General"@en-AU ;
    dct:hasPart F2021L00308:88,
        F2021L00308:89 ;
    dct:isPartOf F2021L00308:84 ;
    dct:isReferencedBy F2021L00308: ;
    rdfs:comment "Division 2 General - Abrievated Graph Key: D87"@en-AU ;
    skos:broader F2021L00308:88,
        F2021L00308:89 ;
    skos:definition "Division 2 General"@en-AU ;
    skos:narrower F2021L00308:84 ;
    skos:prefLabel "Division D87"@en-AU ;
    dcat:accessURL <https://www.legislation.gov.au/F2021L00308/2023-08-04/2023-08-04/text/original/epub/OEBPS/document_1/document_1.html#_Toc143604796> ;
    dcat:landingPage "https://www.legislation.gov.au/F2021L00308/2023-08-04/2023-08-04/text/original/epub/OEBPS/document_1/document_1.html#_Toc143604796"^^xsd:anyURI ;
    dcat:theme legcons:Division .

F2021L00308:112 a legcons:Subdivision,
        owl:Class,
        dcat:Resource ;
    rdfs:label "Subdivision - S112 Subdivision AGeneral requirements"@en-AU ;
    dct:hasPart F2021L00308:113,
        F2021L00308:114,
        F2021L00308:115 ;
    dct:isPartOf F2021L00308:84 ;
    dct:isReferencedBy F2021L00308: ;
    rdfs:comment "Subdivision AGeneral requirements - Abrievated Graph Key: S112"@en-AU ;
    skos:broader F2021L00308:113,
        F2021L00308:114,
        F2021L00308:115 ;
    skos:definition "Subdivision AGeneral requirements"@en-AU ;
    skos:narrower F2021L00308:84 ;
    skos:prefLabel "Subdivision S112"@en-AU ;
    dcat:accessURL <https://www.legislation.gov.au/F2021L00308/2023-08-04/2023-08-04/text/original/epub/OEBPS/document_1/document_1.html#_Toc143604821> ;
    dcat:landingPage "https://www.legislation.gov.au/F2021L00308/2023-08-04/2023-08-04/text/original/epub/OEBPS/document_1/document_1.html#_Toc143604821"^^xsd:anyURI ;
    dcat:theme legcons:Subdivision .

F2021L00308:116 a legcons:Subdivision,
        owl:Class,
        dcat:Resource ;
    rdfs:label "Subdivision - S116 Subdivision BRequirements for prescribed rabbit meat and prescribed rabbit meat products carcases and carcase parts"@en-AU ;
    dct:hasPart F2021L00308:117,
        F2021L00308:118,
        F2021L00308:119 ;
    dct:isPartOf F2021L00308:84 ;
    dct:isReferencedBy F2021L00308: ;
    rdfs:comment "Subdivision BRequirements for prescribed rabbit meat and prescribed rabbit meat products carcases and carcase parts - Abrievated Graph Key: S116"@en-AU ;
    skos:broader F2021L00308:117,
        F2021L00308:118,
        F2021L00308:119 ;
    skos:definition "Subdivision BRequirements for prescribed rabbit meat and prescribed rabbit meat products carcases and carcase parts"@en-AU ;
    skos:narrower F2021L00308:84 ;
    skos:prefLabel "Subdivision S116"@en-AU ;
    dcat:accessURL <https://www.legislation.gov.au/F2021L00308/2023-08-04/2023-08-04/text/original/epub/OEBPS/document_1/document_1.html#_Toc143604825> ;
    dcat:landingPage "https://www.legislation.gov.au/F2021L00308/2023-08-04/2023-08-04/text/original/epub/OEBPS/document_1/document_1.html#_Toc143604825"^^xsd:anyURI ;
    dcat:theme legcons:Subdivision .

F2021L00308:157 a legcons:Part,
        owl:Class,
        dcat:Resource ;
    rdfs:label "Part - P157 Part 2 Variation suspension and revocation of export permit"@en-AU ;
    dct:hasPart F2021L00308:158,
        F2021L00308:159,
        F2021L00308:160 ;
    dct:isPartOf F2021L00308:154 ;
    dct:isReferencedBy F2021L00308: ;
    rdfs:comment "Part 2 Variation suspension and revocation of export permit - Abrievated Graph Key: P157"@en-AU ;
    skos:broader F2021L00308:158,
        F2021L00308:159,
        F2021L00308:160 ;
    skos:definition "Part 2 Variation suspension and revocation of export permit"@en-AU ;
    skos:narrower F2021L00308:154 ;
    skos:prefLabel "Part P157"@en-AU ;
    dcat:accessURL <https://www.legislation.gov.au/F2021L00308/2023-08-04/2023-08-04/text/original/epub/OEBPS/document_1/document_1.html#_Toc143604866> ;
    dcat:landingPage "https://www.legislation.gov.au/F2021L00308/2023-08-04/2023-08-04/text/original/epub/OEBPS/document_1/document_1.html#_Toc143604866"^^xsd:anyURI ;
    dcat:theme legcons:Part .

F2021L00308:172 a legcons:Part,
        owl:Class,
        dcat:Resource ;
    rdfs:label "Part - P172 Part 2 Trade descriptions"@en-AU ;
    dct:hasPart F2021L00308:173,
        F2021L00308:174,
        F2021L00308:175 ;
    dct:isPartOf F2021L00308:166 ;
    dct:isReferencedBy F2021L00308: ;
    rdfs:comment "Part 2 Trade descriptions - Abrievated Graph Key: P172"@en-AU ;
    skos:broader F2021L00308:173,
        F2021L00308:174,
        F2021L00308:175 ;
    skos:definition "Part 2 Trade descriptions"@en-AU ;
    skos:narrower F2021L00308:166 ;
    skos:prefLabel "Part P172"@en-AU ;
    dcat:accessURL <https://www.legislation.gov.au/F2021L00308/2023-08-04/2023-08-04/text/original/epub/OEBPS/document_1/document_1.html#_Toc143604881> ;
    dcat:landingPage "https://www.legislation.gov.au/F2021L00308/2023-08-04/2023-08-04/text/original/epub/OEBPS/document_1/document_1.html#_Toc143604881"^^xsd:anyURI ;
    dcat:theme legcons:Part .

F2021L00308:201 a legcons:Division,
        owl:Class,
        dcat:Resource ;
    rdfs:label "Division - D201 Division 3 Marks resembling official marks"@en-AU ;
    dct:hasPart F2021L00308:202,
        F2021L00308:203,
        F2021L00308:204 ;
    dct:isPartOf F2021L00308:176 ;
    dct:isReferencedBy F2021L00308: ;
    rdfs:comment "Division 3 Marks resembling official marks - Abrievated Graph Key: D201"@en-AU ;
    skos:broader F2021L00308:202,
        F2021L00308:203,
        F2021L00308:204 ;
    skos:definition "Division 3 Marks resembling official marks"@en-AU ;
    skos:narrower F2021L00308:176 ;
    skos:prefLabel "Division D201"@en-AU ;
    dcat:accessURL <https://www.legislation.gov.au/F2021L00308/2023-08-04/2023-08-04/text/original/epub/OEBPS/document_1/document_1.html#_Toc143604910> ;
    dcat:landingPage "https://www.legislation.gov.au/F2021L00308/2023-08-04/2023-08-04/text/original/epub/OEBPS/document_1/document_1.html#_Toc143604910"^^xsd:anyURI ;
    dcat:theme legcons:Division .

F2021L00308:212 a legcons:Chapter,
        owl:Class,
        dcat:Resource ;
    rdfs:label "Chapter - C212 Chapter 9 Powers and officials"@en-AU ;
    dct:hasPart F2021L00308:213,
        F2021L00308:233,
        F2021L00308:235,
        F2021L00308:237 ;
    dct:isReferencedBy F2021L00308: ;
    rdfs:comment "Chapter 9 Powers and officials - Abrievated Graph Key: C212"@en-AU ;
    skos:broader F2021L00308:213,
        F2021L00308:233,
        F2021L00308:235,
        F2021L00308:237 ;
    skos:definition "Chapter 9 Powers and officials"@en-AU ;
    skos:prefLabel "Chapter C212"@en-AU ;
    dcat:accessURL <https://www.legislation.gov.au/F2021L00308/2023-08-04/2023-08-04/text/original/epub/OEBPS/document_1/document_1.html#_Toc143604921> ;
    dcat:landingPage "https://www.legislation.gov.au/F2021L00308/2023-08-04/2023-08-04/text/original/epub/OEBPS/document_1/document_1.html#_Toc143604921"^^xsd:anyURI ;
    dcat:theme legcons:Chapter .

F2021L00308:213 a legcons:Part,
        owl:Class,
        dcat:Resource ;
    rdfs:label "Part - P213 Part 1 Audits"@en-AU ;
    dct:hasPart F2021L00308:214,
        F2021L00308:216,
        F2021L00308:221 ;
    dct:isPartOf F2021L00308:212 ;
    dct:isReferencedBy F2021L00308: ;
    rdfs:comment "Part 1 Audits - Abrievated Graph Key: P213"@en-AU ;
    skos:broader F2021L00308:214,
        F2021L00308:216,
        F2021L00308:221 ;
    skos:definition "Part 1 Audits"@en-AU ;
    skos:narrower F2021L00308:212 ;
    skos:prefLabel "Part P213"@en-AU ;
    dcat:accessURL <https://www.legislation.gov.au/F2021L00308/2023-08-04/2023-08-04/text/original/epub/OEBPS/document_1/document_1.html#_Toc143604922> ;
    dcat:landingPage "https://www.legislation.gov.au/F2021L00308/2023-08-04/2023-08-04/text/original/epub/OEBPS/document_1/document_1.html#_Toc143604922"^^xsd:anyURI ;
    dcat:theme legcons:Part .

F2021L00308:289 a legcons:Division,
        owl:Class,
        dcat:Resource ;
    rdfs:label "Division - D289 Division 1 Official marks"@en-AU ;
    dct:hasPart F2021L00308:290,
        F2021L00308:291,
        F2021L00308:292 ;
    dct:isPartOf F2021L00308:288 ;
    dct:isReferencedBy F2021L00308: ;
    rdfs:comment "Division 1 Official marks - Abrievated Graph Key: D289"@en-AU ;
    skos:broader F2021L00308:290,
        F2021L00308:291,
        F2021L00308:292 ;
    skos:definition "Division 1 Official marks"@en-AU ;
    skos:narrower F2021L00308:288 ;
    skos:prefLabel "Division D289"@en-AU ;
    dcat:accessURL <https://www.legislation.gov.au/F2021L00308/2023-08-04/2023-08-04/text/original/epub/OEBPS/document_1/document_1.html#_Toc143604998> ;
    dcat:landingPage "https://www.legislation.gov.au/F2021L00308/2023-08-04/2023-08-04/text/original/epub/OEBPS/document_1/document_1.html#_Toc143604998"^^xsd:anyURI ;
    dcat:theme legcons:Division .

F2021L00308:60 a legcons:Part,
        owl:Class,
        dcat:Resource ;
    rdfs:label "Part - P60 Part 5 Matters relating to applications"@en-AU ;
    dct:hasPart F2021L00308:61,
        F2021L00308:62,
        F2021L00308:63 ;
    dct:isPartOf F2021L00308:35 ;
    dct:isReferencedBy F2021L00308: ;
    rdfs:comment "Part 5 Matters relating to applications - Abrievated Graph Key: P60"@en-AU ;
    skos:broader F2021L00308:61,
        F2021L00308:62,
        F2021L00308:63 ;
    skos:definition "Part 5 Matters relating to applications"@en-AU ;
    skos:narrower F2021L00308:35 ;
    skos:prefLabel "Part P60"@en-AU ;
    dcat:accessURL <https://www.legislation.gov.au/F2021L00308/2023-08-04/2023-08-04/text/original/epub/OEBPS/document_1/document_1.html#_Toc143604769> ;
    dcat:landingPage "https://www.legislation.gov.au/F2021L00308/2023-08-04/2023-08-04/text/original/epub/OEBPS/document_1/document_1.html#_Toc143604769"^^xsd:anyURI ;
    dcat:theme legcons:Part .

F2021L00308:91 a legcons:Subdivision,
        owl:Class,
        dcat:Resource ;
    rdfs:label "Subdivision - S91 Subdivision AGeneral"@en-AU ;
    dct:hasPart F2021L00308:92,
        F2021L00308:93,
        F2021L00308:94 ;
    dct:isPartOf F2021L00308:90 ;
    dct:isReferencedBy F2021L00308: ;
    rdfs:comment "Subdivision AGeneral - Abrievated Graph Key: S91"@en-AU ;
    skos:broader F2021L00308:92,
        F2021L00308:93,
        F2021L00308:94 ;
    skos:definition "Subdivision AGeneral"@en-AU ;
    skos:narrower F2021L00308:90 ;
    skos:prefLabel "Subdivision S91"@en-AU ;
    dcat:accessURL <https://www.legislation.gov.au/F2021L00308/2023-08-04/2023-08-04/text/original/epub/OEBPS/document_1/document_1.html#_Toc143604800> ;
    dcat:landingPage "https://www.legislation.gov.au/F2021L00308/2023-08-04/2023-08-04/text/original/epub/OEBPS/document_1/document_1.html#_Toc143604800"^^xsd:anyURI ;
    dcat:theme legcons:Subdivision .

F2021L00308:161 a legcons:Part,
        owl:Class,
        dcat:Resource ;
    rdfs:label "Part - P161 Part 3 Other matters"@en-AU ;
    dct:hasPart F2021L00308:162,
        F2021L00308:163,
        F2021L00308:164,
        F2021L00308:165 ;
    dct:isPartOf F2021L00308:154 ;
    dct:isReferencedBy F2021L00308: ;
    rdfs:comment "Part 3 Other matters - Abrievated Graph Key: P161"@en-AU ;
    skos:broader F2021L00308:162,
        F2021L00308:163,
        F2021L00308:164,
        F2021L00308:165 ;
    skos:definition "Part 3 Other matters"@en-AU ;
    skos:narrower F2021L00308:154 ;
    skos:prefLabel "Part P161"@en-AU ;
    dcat:accessURL <https://www.legislation.gov.au/F2021L00308/2023-08-04/2023-08-04/text/original/epub/OEBPS/document_1/document_1.html#_Toc143604870> ;
    dcat:landingPage "https://www.legislation.gov.au/F2021L00308/2023-08-04/2023-08-04/text/original/epub/OEBPS/document_1/document_1.html#_Toc143604870"^^xsd:anyURI ;
    dcat:theme legcons:Part .

F2021L00308:167 a legcons:Part,
        owl:Class,
        dcat:Resource ;
    rdfs:label "Part - P167 Part 1 Notices of intention to export"@en-AU ;
    dct:hasPart F2021L00308:168,
        F2021L00308:169,
        F2021L00308:170,
        F2021L00308:171 ;
    dct:isPartOf F2021L00308:166 ;
    dct:isReferencedBy F2021L00308: ;
    rdfs:comment "Part 1 Notices of intention to export - Abrievated Graph Key: P167"@en-AU ;
    skos:broader F2021L00308:168,
        F2021L00308:169,
        F2021L00308:170,
        F2021L00308:171 ;
    skos:definition "Part 1 Notices of intention to export"@en-AU ;
    skos:narrower F2021L00308:166 ;
    skos:prefLabel "Part P167"@en-AU ;
    dcat:accessURL <https://www.legislation.gov.au/F2021L00308/2023-08-04/2023-08-04/text/original/epub/OEBPS/document_1/document_1.html#_Toc143604876> ;
    dcat:landingPage "https://www.legislation.gov.au/F2021L00308/2023-08-04/2023-08-04/text/original/epub/OEBPS/document_1/document_1.html#_Toc143604876"^^xsd:anyURI ;
    dcat:theme legcons:Part .

F2021L00308:176 a legcons:Part,
        owl:Class,
        dcat:Resource ;
    rdfs:label "Part - P176 Part 3 Official marks"@en-AU ;
    dct:hasPart F2021L00308:177,
        F2021L00308:188,
        F2021L00308:201,
        F2021L00308:205 ;
    dct:isPartOf F2021L00308:166 ;
    dct:isReferencedBy F2021L00308: ;
    rdfs:comment "Part 3 Official marks - Abrievated Graph Key: P176"@en-AU ;
    skos:broader F2021L00308:177,
        F2021L00308:188,
        F2021L00308:201,
        F2021L00308:205 ;
    skos:definition "Part 3 Official marks"@en-AU ;
    skos:narrower F2021L00308:166 ;
    skos:prefLabel "Part P176"@en-AU ;
    dcat:accessURL <https://www.legislation.gov.au/F2021L00308/2023-08-04/2023-08-04/text/original/epub/OEBPS/document_1/document_1.html#_Toc143604885> ;
    dcat:landingPage "https://www.legislation.gov.au/F2021L00308/2023-08-04/2023-08-04/text/original/epub/OEBPS/document_1/document_1.html#_Toc143604885"^^xsd:anyURI ;
    dcat:theme legcons:Part .

F2021L00308:216 a legcons:Division,
        owl:Class,
        dcat:Resource ;
    rdfs:label "Division - D216 Division 2 Conduct of audit etc"@en-AU ;
    dct:hasPart F2021L00308:217,
        F2021L00308:218,
        F2021L00308:219,
        F2021L00308:220 ;
    dct:isPartOf F2021L00308:213 ;
    dct:isReferencedBy F2021L00308: ;
    rdfs:comment "Division 2 Conduct of audit etc - Abrievated Graph Key: D216"@en-AU ;
    skos:broader F2021L00308:217,
        F2021L00308:218,
        F2021L00308:219,
        F2021L00308:220 ;
    skos:definition "Division 2 Conduct of audit etc"@en-AU ;
    skos:narrower F2021L00308:213 ;
    skos:prefLabel "Division D216"@en-AU ;
    dcat:accessURL <https://www.legislation.gov.au/F2021L00308/2023-08-04/2023-08-04/text/original/epub/OEBPS/document_1/document_1.html#_Toc143604925> ;
    dcat:landingPage "https://www.legislation.gov.au/F2021L00308/2023-08-04/2023-08-04/text/original/epub/OEBPS/document_1/document_1.html#_Toc143604925"^^xsd:anyURI ;
    dcat:theme legcons:Division .

F2021L00308:237 a legcons:Part,
        owl:Class,
        dcat:Resource ;
    rdfs:label "Part - P237 Part 4 Authorised officers"@en-AU ;
    dct:hasPart F2021L00308:238,
        F2021L00308:240,
        F2021L00308:257,
        F2021L00308:259 ;
    dct:isPartOf F2021L00308:212 ;
    dct:isReferencedBy F2021L00308: ;
    rdfs:comment "Part 4 Authorised officers - Abrievated Graph Key: P237"@en-AU ;
    skos:broader F2021L00308:238,
        F2021L00308:240,
        F2021L00308:257,
        F2021L00308:259 ;
    skos:definition "Part 4 Authorised officers"@en-AU ;
    skos:narrower F2021L00308:212 ;
    skos:prefLabel "Part P237"@en-AU ;
    dcat:accessURL <https://www.legislation.gov.au/F2021L00308/2023-08-04/2023-08-04/text/original/epub/OEBPS/document_1/document_1.html#_Toc143604946> ;
    dcat:landingPage "https://www.legislation.gov.au/F2021L00308/2023-08-04/2023-08-04/text/original/epub/OEBPS/document_1/document_1.html#_Toc143604946"^^xsd:anyURI ;
    dcat:theme legcons:Part .

F2021L00308:264 a legcons:Chapter,
        owl:Class,
        dcat:Resource ;
    rdfs:label "Chapter - C264 Chapter 11 Miscellaneous"@en-AU ;
    dct:hasPart F2021L00308:265,
        F2021L00308:267,
        F2021L00308:278,
        F2021L00308:280,
        F2021L00308:283 ;
    dct:isReferencedBy F2021L00308: ;
    rdfs:comment "Chapter 11 Miscellaneous - Abrievated Graph Key: C264"@en-AU ;
    skos:broader F2021L00308:265,
        F2021L00308:267,
        F2021L00308:278,
        F2021L00308:280,
        F2021L00308:283 ;
    skos:definition "Chapter 11 Miscellaneous"@en-AU ;
    skos:prefLabel "Chapter C264"@en-AU ;
    dcat:accessURL <https://www.legislation.gov.au/F2021L00308/2023-08-04/2023-08-04/text/original/epub/OEBPS/document_1/document_1.html#_Toc143604973> ;
    dcat:landingPage "https://www.legislation.gov.au/F2021L00308/2023-08-04/2023-08-04/text/original/epub/OEBPS/document_1/document_1.html#_Toc143604973"^^xsd:anyURI ;
    dcat:theme legcons:Chapter .

F2021L00308:303 a legcons:Endnotes,
        owl:Class,
        dcat:Resource ;
    rdfs:label "Endnotes - E303 Endnotes"@en-AU ;
    dct:hasPart F2021L00308:304,
        F2021L00308:305,
        F2021L00308:306,
        F2021L00308:307 ;
    dct:isPartOf F2021L00308:298 ;
    dct:isReferencedBy F2021L00308: ;
    rdfs:comment "Endnotes - Abrievated Graph Key: E303"@en-AU ;
    skos:broader F2021L00308:304,
        F2021L00308:305,
        F2021L00308:306,
        F2021L00308:307 ;
    skos:definition "Endnotes"@en-AU ;
    skos:narrower F2021L00308:298 ;
    skos:prefLabel "Endnotes E303"@en-AU ;
    dcat:accessURL <https://www.legislation.gov.au/F2021L00308/2023-08-04/2023-08-04/text/original/epub/OEBPS/document_1/document_1.html#_Toc143605012> ;
    dcat:landingPage "https://www.legislation.gov.au/F2021L00308/2023-08-04/2023-08-04/text/original/epub/OEBPS/document_1/document_1.html#_Toc143605012"^^xsd:anyURI ;
    dcat:theme legcons:Endnotes .

F2021L00308:29 a legcons:Part,
        owl:Class,
        dcat:Resource ;
    rdfs:label "Part - P29 Part 3 Government certificates"@en-AU ;
    dct:hasPart F2021L00308:30,
        F2021L00308:31,
        F2021L00308:32,
        F2021L00308:33,
        F2021L00308:34 ;
    dct:isPartOf F2021L00308:14 ;
    dct:isReferencedBy F2021L00308: ;
    rdfs:comment "Part 3 Government certificates - Abrievated Graph Key: P29"@en-AU ;
    skos:broader F2021L00308:30,
        F2021L00308:31,
        F2021L00308:32,
        F2021L00308:33,
        F2021L00308:34 ;
    skos:definition "Part 3 Government certificates"@en-AU ;
    skos:narrower F2021L00308:14 ;
    skos:prefLabel "Part P29"@en-AU ;
    dcat:accessURL <https://www.legislation.gov.au/F2021L00308/2023-08-04/2023-08-04/text/original/epub/OEBPS/document_1/document_1.html#_Toc143604738> ;
    dcat:landingPage "https://www.legislation.gov.au/F2021L00308/2023-08-04/2023-08-04/text/original/epub/OEBPS/document_1/document_1.html#_Toc143604738"^^xsd:anyURI ;
    dcat:theme legcons:Part .

F2021L00308:35 a legcons:Chapter,
        owl:Class,
        dcat:Resource ;
    rdfs:label "Chapter - C35 Chapter 4 Registered establishments"@en-AU ;
    dct:hasPart F2021L00308:36,
        F2021L00308:48,
        F2021L00308:55,
        F2021L00308:58,
        F2021L00308:60,
        F2021L00308:64 ;
    dct:isReferencedBy F2021L00308: ;
    rdfs:comment "Chapter 4 Registered establishments - Abrievated Graph Key: C35"@en-AU ;
    skos:broader F2021L00308:36,
        F2021L00308:48,
        F2021L00308:55,
        F2021L00308:58,
        F2021L00308:60,
        F2021L00308:64 ;
    skos:definition "Chapter 4 Registered establishments"@en-AU ;
    skos:prefLabel "Chapter C35"@en-AU ;
    dcat:accessURL <https://www.legislation.gov.au/F2021L00308/2023-08-04/2023-08-04/text/original/epub/OEBPS/document_1/document_1.html#_Toc143604744> ;
    dcat:landingPage "https://www.legislation.gov.au/F2021L00308/2023-08-04/2023-08-04/text/original/epub/OEBPS/document_1/document_1.html#_Toc143604744"^^xsd:anyURI ;
    dcat:theme legcons:Chapter .

F2021L00308:74 a legcons:Division,
        owl:Class,
        dcat:Resource ;
    rdfs:label "Division - D74 Division 2 Variation of meat inspection services"@en-AU ;
    dct:hasPart F2021L00308:75,
        F2021L00308:76,
        F2021L00308:77,
        F2021L00308:78,
        F2021L00308:79 ;
    dct:isPartOf F2021L00308:64 ;
    dct:isReferencedBy F2021L00308: ;
    rdfs:comment "Division 2 Variation of meat inspection services - Abrievated Graph Key: D74"@en-AU ;
    skos:broader F2021L00308:75,
        F2021L00308:76,
        F2021L00308:77,
        F2021L00308:78,
        F2021L00308:79 ;
    skos:definition "Division 2 Variation of meat inspection services"@en-AU ;
    skos:narrower F2021L00308:64 ;
    skos:prefLabel "Division D74"@en-AU ;
    dcat:accessURL <https://www.legislation.gov.au/F2021L00308/2023-08-04/2023-08-04/text/original/epub/OEBPS/document_1/document_1.html#_Toc143604783> ;
    dcat:landingPage "https://www.legislation.gov.au/F2021L00308/2023-08-04/2023-08-04/text/original/epub/OEBPS/document_1/document_1.html#_Toc143604783"^^xsd:anyURI ;
    dcat:theme legcons:Division .

F2021L00308:205 a legcons:Division,
        owl:Class,
        dcat:Resource ;
    rdfs:label "Division - D205 Division 4 Official marking devices"@en-AU ;
    dct:hasPart F2021L00308:206,
        F2021L00308:207,
        F2021L00308:208,
        F2021L00308:209,
        F2021L00308:210,
        F2021L00308:211 ;
    dct:isPartOf F2021L00308:176 ;
    dct:isReferencedBy F2021L00308: ;
    rdfs:comment "Division 4 Official marking devices - Abrievated Graph Key: D205"@en-AU ;
    skos:broader F2021L00308:206,
        F2021L00308:207,
        F2021L00308:208,
        F2021L00308:209,
        F2021L00308:210,
        F2021L00308:211 ;
    skos:definition "Division 4 Official marking devices"@en-AU ;
    skos:narrower F2021L00308:176 ;
    skos:prefLabel "Division D205"@en-AU ;
    dcat:accessURL <https://www.legislation.gov.au/F2021L00308/2023-08-04/2023-08-04/text/original/epub/OEBPS/document_1/document_1.html#_Toc143604914> ;
    dcat:landingPage "https://www.legislation.gov.au/F2021L00308/2023-08-04/2023-08-04/text/original/epub/OEBPS/document_1/document_1.html#_Toc143604914"^^xsd:anyURI ;
    dcat:theme legcons:Division .

F2021L00308:22 a legcons:Part,
        owl:Class,
        dcat:Resource ;
    rdfs:label "Part - P22 Part 2 Exemptions"@en-AU ;
    dct:hasPart F2021L00308:23,
        F2021L00308:24,
        F2021L00308:25,
        F2021L00308:26,
        F2021L00308:27,
        F2021L00308:28 ;
    dct:isPartOf F2021L00308:14 ;
    dct:isReferencedBy F2021L00308: ;
    rdfs:comment "Part 2 Exemptions - Abrievated Graph Key: P22"@en-AU ;
    skos:broader F2021L00308:23,
        F2021L00308:24,
        F2021L00308:25,
        F2021L00308:26,
        F2021L00308:27,
        F2021L00308:28 ;
    skos:definition "Part 2 Exemptions"@en-AU ;
    skos:narrower F2021L00308:14 ;
    skos:prefLabel "Part P22"@en-AU ;
    dcat:accessURL <https://www.legislation.gov.au/F2021L00308/2023-08-04/2023-08-04/text/original/epub/OEBPS/document_1/document_1.html#_Toc143604731> ;
    dcat:landingPage "https://www.legislation.gov.au/F2021L00308/2023-08-04/2023-08-04/text/original/epub/OEBPS/document_1/document_1.html#_Toc143604731"^^xsd:anyURI ;
    dcat:theme legcons:Part .

F2021L00308:48 a legcons:Part,
        owl:Class,
        dcat:Resource ;
    rdfs:label "Part - P48 Part 2 Conditions of registration"@en-AU ;
    dct:hasPart F2021L00308:49,
        F2021L00308:50,
        F2021L00308:51,
        F2021L00308:52,
        F2021L00308:53,
        F2021L00308:54 ;
    dct:isPartOf F2021L00308:35 ;
    dct:isReferencedBy F2021L00308: ;
    rdfs:comment "Part 2 Conditions of registration - Abrievated Graph Key: P48"@en-AU ;
    skos:broader F2021L00308:49,
        F2021L00308:50,
        F2021L00308:51,
        F2021L00308:52,
        F2021L00308:53,
        F2021L00308:54 ;
    skos:definition "Part 2 Conditions of registration"@en-AU ;
    skos:narrower F2021L00308:35 ;
    skos:prefLabel "Part P48"@en-AU ;
    dcat:accessURL <https://www.legislation.gov.au/F2021L00308/2023-08-04/2023-08-04/text/original/epub/OEBPS/document_1/document_1.html#_Toc143604757> ;
    dcat:landingPage "https://www.legislation.gov.au/F2021L00308/2023-08-04/2023-08-04/text/original/epub/OEBPS/document_1/document_1.html#_Toc143604757"^^xsd:anyURI ;
    dcat:theme legcons:Part .

F2021L00308:65 a legcons:Division,
        owl:Class,
        dcat:Resource ;
    rdfs:label "Division - D65 Division 1 Allocation of meat inspection services"@en-AU ;
    dct:hasPart F2021L00308:66,
        F2021L00308:67,
        F2021L00308:68,
        F2021L00308:69,
        F2021L00308:70,
        F2021L00308:71,
        F2021L00308:72,
        F2021L00308:73 ;
    dct:isPartOf F2021L00308:64 ;
    dct:isReferencedBy F2021L00308: ;
    rdfs:comment "Division 1 Allocation of meat inspection services - Abrievated Graph Key: D65"@en-AU ;
    skos:broader F2021L00308:66,
        F2021L00308:67,
        F2021L00308:68,
        F2021L00308:69,
        F2021L00308:70,
        F2021L00308:71,
        F2021L00308:72,
        F2021L00308:73 ;
    skos:definition "Division 1 Allocation of meat inspection services"@en-AU ;
    skos:narrower F2021L00308:64 ;
    skos:prefLabel "Division D65"@en-AU ;
    dcat:accessURL <https://www.legislation.gov.au/F2021L00308/2023-08-04/2023-08-04/text/original/epub/OEBPS/document_1/document_1.html#_Toc143604774> ;
    dcat:landingPage "https://www.legislation.gov.au/F2021L00308/2023-08-04/2023-08-04/text/original/epub/OEBPS/document_1/document_1.html#_Toc143604774"^^xsd:anyURI ;
    dcat:theme legcons:Division .

F2021L00308:177 a legcons:Division,
        owl:Class,
        dcat:Resource ;
    rdfs:label "Division - D177 Division 1 Marks that are official marks"@en-AU ;
    dct:hasPart F2021L00308:178,
        F2021L00308:179,
        F2021L00308:180,
        F2021L00308:181,
        F2021L00308:182,
        F2021L00308:183,
        F2021L00308:184,
        F2021L00308:185,
        F2021L00308:186,
        F2021L00308:187 ;
    dct:isPartOf F2021L00308:176 ;
    dct:isReferencedBy F2021L00308: ;
    rdfs:comment "Division 1 Marks that are official marks - Abrievated Graph Key: D177"@en-AU ;
    skos:broader F2021L00308:178,
        F2021L00308:179,
        F2021L00308:180,
        F2021L00308:181,
        F2021L00308:182,
        F2021L00308:183,
        F2021L00308:184,
        F2021L00308:185,
        F2021L00308:186,
        F2021L00308:187 ;
    skos:definition "Division 1 Marks that are official marks"@en-AU ;
    skos:narrower F2021L00308:176 ;
    skos:prefLabel "Division D177"@en-AU ;
    dcat:accessURL <https://www.legislation.gov.au/F2021L00308/2023-08-04/2023-08-04/text/original/epub/OEBPS/document_1/document_1.html#_Toc143604886> ;
    dcat:landingPage "https://www.legislation.gov.au/F2021L00308/2023-08-04/2023-08-04/text/original/epub/OEBPS/document_1/document_1.html#_Toc143604886"^^xsd:anyURI ;
    dcat:theme legcons:Division .

F2021L00308:267 a legcons:Part,
        owl:Class,
        dcat:Resource ;
    rdfs:label "Part - P267 Part 2 Records"@en-AU ;
    dct:hasPart F2021L00308:268,
        F2021L00308:269,
        F2021L00308:270,
        F2021L00308:271,
        F2021L00308:272,
        F2021L00308:273,
        F2021L00308:274,
        F2021L00308:275,
        F2021L00308:276,
        F2021L00308:277 ;
    dct:isPartOf F2021L00308:264 ;
    dct:isReferencedBy F2021L00308: ;
    rdfs:comment "Part 2 Records - Abrievated Graph Key: P267"@en-AU ;
    skos:broader F2021L00308:268,
        F2021L00308:269,
        F2021L00308:270,
        F2021L00308:271,
        F2021L00308:272,
        F2021L00308:273,
        F2021L00308:274,
        F2021L00308:275,
        F2021L00308:276,
        F2021L00308:277 ;
    skos:definition "Part 2 Records"@en-AU ;
    skos:narrower F2021L00308:264 ;
    skos:prefLabel "Part P267"@en-AU ;
    dcat:accessURL <https://www.legislation.gov.au/F2021L00308/2023-08-04/2023-08-04/text/original/epub/OEBPS/document_1/document_1.html#_Toc143604976> ;
    dcat:landingPage "https://www.legislation.gov.au/F2021L00308/2023-08-04/2023-08-04/text/original/epub/OEBPS/document_1/document_1.html#_Toc143604976"^^xsd:anyURI ;
    dcat:theme legcons:Part .

F2021L00308:80 a legcons:Chapter,
        owl:Class,
        dcat:Resource ;
    rdfs:label "Chapter - C80 Chapter 5 Approved arrangements"@en-AU ;
    dct:hasPart F2021L00308:142,
        F2021L00308:143,
        F2021L00308:144,
        F2021L00308:145,
        F2021L00308:148,
        F2021L00308:150,
        F2021L00308:151,
        F2021L00308:152,
        F2021L00308:153,
        F2021L00308:81,
        F2021L00308:84 ;
    dct:isReferencedBy F2021L00308: ;
    rdfs:comment "Chapter 5 Approved arrangements - Abrievated Graph Key: C80"@en-AU ;
    skos:broader F2021L00308:142,
        F2021L00308:143,
        F2021L00308:144,
        F2021L00308:145,
        F2021L00308:148,
        F2021L00308:150,
        F2021L00308:151,
        F2021L00308:152,
        F2021L00308:153,
        F2021L00308:81,
        F2021L00308:84 ;
    skos:definition "Chapter 5 Approved arrangements"@en-AU ;
    skos:prefLabel "Chapter C80"@en-AU ;
    dcat:accessURL <https://www.legislation.gov.au/F2021L00308/2023-08-04/2023-08-04/text/original/epub/OEBPS/document_1/document_1.html#_Toc143604789> ;
    dcat:landingPage "https://www.legislation.gov.au/F2021L00308/2023-08-04/2023-08-04/text/original/epub/OEBPS/document_1/document_1.html#_Toc143604789"^^xsd:anyURI ;
    dcat:theme legcons:Chapter .

F2021L00308:90 a legcons:Division,
        owl:Class,
        dcat:Resource ;
    rdfs:label "Division - D90 Division 3 Preparation"@en-AU ;
    dct:hasPart F2021L00308:100,
        F2021L00308:101,
        F2021L00308:102,
        F2021L00308:103,
        F2021L00308:91,
        F2021L00308:95,
        F2021L00308:96,
        F2021L00308:97,
        F2021L00308:98,
        F2021L00308:99 ;
    dct:isPartOf F2021L00308:84 ;
    dct:isReferencedBy F2021L00308: ;
    rdfs:comment "Division 3 Preparation - Abrievated Graph Key: D90"@en-AU ;
    skos:broader F2021L00308:100,
        F2021L00308:101,
        F2021L00308:102,
        F2021L00308:103,
        F2021L00308:91,
        F2021L00308:95,
        F2021L00308:96,
        F2021L00308:97,
        F2021L00308:98,
        F2021L00308:99 ;
    skos:definition "Division 3 Preparation"@en-AU ;
    skos:narrower F2021L00308:84 ;
    skos:prefLabel "Division D90"@en-AU ;
    dcat:accessURL <https://www.legislation.gov.au/F2021L00308/2023-08-04/2023-08-04/text/original/epub/OEBPS/document_1/document_1.html#_Toc143604799> ;
    dcat:landingPage "https://www.legislation.gov.au/F2021L00308/2023-08-04/2023-08-04/text/original/epub/OEBPS/document_1/document_1.html#_Toc143604799"^^xsd:anyURI ;
    dcat:theme legcons:Division .

F2021L00308:1 a legcons:Chapter,
        owl:Class,
        dcat:Resource ;
    rdfs:label "Chapter - C1 Chapter 1 Preliminary"@en-AU ;
    dct:hasPart F2021L00308:10,
        F2021L00308:11,
        F2021L00308:12,
        F2021L00308:13,
        F2021L00308:2,
        F2021L00308:3,
        F2021L00308:4,
        F2021L00308:5,
        F2021L00308:6,
        F2021L00308:7,
        F2021L00308:8,
        F2021L00308:9 ;
    dct:isReferencedBy F2021L00308: ;
    rdfs:comment "Chapter 1 Preliminary - Abrievated Graph Key: C1"@en-AU ;
    skos:broader F2021L00308:10,
        F2021L00308:11,
        F2021L00308:12,
        F2021L00308:13,
        F2021L00308:2,
        F2021L00308:3,
        F2021L00308:4,
        F2021L00308:5,
        F2021L00308:6,
        F2021L00308:7,
        F2021L00308:8,
        F2021L00308:9 ;
    skos:definition "Chapter 1 Preliminary"@en-AU ;
    skos:prefLabel "Chapter C1"@en-AU ;
    dcat:accessURL <https://www.legislation.gov.au/F2021L00308/2023-08-04/2023-08-04/text/original/epub/OEBPS/document_1/document_1.html#_Toc143604710> ;
    dcat:landingPage "https://www.legislation.gov.au/F2021L00308/2023-08-04/2023-08-04/text/original/epub/OEBPS/document_1/document_1.html#_Toc143604710"^^xsd:anyURI ;
    dcat:theme legcons:Chapter .

F2021L00308:221 a legcons:Division,
        owl:Class,
        dcat:Resource ;
    rdfs:label "Division - D221 Division 3 Approved auditors"@en-AU ;
    dct:hasPart F2021L00308:222,
        F2021L00308:223,
        F2021L00308:224,
        F2021L00308:225,
        F2021L00308:226,
        F2021L00308:227,
        F2021L00308:228,
        F2021L00308:229,
        F2021L00308:230,
        F2021L00308:231,
        F2021L00308:232 ;
    dct:isPartOf F2021L00308:213 ;
    dct:isReferencedBy F2021L00308: ;
    rdfs:comment "Division 3 Approved auditors - Abrievated Graph Key: D221"@en-AU ;
    skos:broader F2021L00308:222,
        F2021L00308:223,
        F2021L00308:224,
        F2021L00308:225,
        F2021L00308:226,
        F2021L00308:227,
        F2021L00308:228,
        F2021L00308:229,
        F2021L00308:230,
        F2021L00308:231,
        F2021L00308:232 ;
    skos:definition "Division 3 Approved auditors"@en-AU ;
    skos:narrower F2021L00308:213 ;
    skos:prefLabel "Division D221"@en-AU ;
    dcat:accessURL <https://www.legislation.gov.au/F2021L00308/2023-08-04/2023-08-04/text/original/epub/OEBPS/document_1/document_1.html#_Toc143604930> ;
    dcat:landingPage "https://www.legislation.gov.au/F2021L00308/2023-08-04/2023-08-04/text/original/epub/OEBPS/document_1/document_1.html#_Toc143604930"^^xsd:anyURI ;
    dcat:theme legcons:Division .

F2021L00308:36 a legcons:Part,
        owl:Class,
        dcat:Resource ;
    rdfs:label "Part - P36 Part 1 Requirements for registration"@en-AU ;
    dct:hasPart F2021L00308:37,
        F2021L00308:38,
        F2021L00308:39,
        F2021L00308:40,
        F2021L00308:41,
        F2021L00308:42,
        F2021L00308:43,
        F2021L00308:44,
        F2021L00308:45,
        F2021L00308:46,
        F2021L00308:47 ;
    dct:isPartOf F2021L00308:35 ;
    dct:isReferencedBy F2021L00308: ;
    rdfs:comment "Part 1 Requirements for registration - Abrievated Graph Key: P36"@en-AU ;
    skos:broader F2021L00308:37,
        F2021L00308:38,
        F2021L00308:39,
        F2021L00308:40,
        F2021L00308:41,
        F2021L00308:42,
        F2021L00308:43,
        F2021L00308:44,
        F2021L00308:45,
        F2021L00308:46,
        F2021L00308:47 ;
    skos:definition "Part 1 Requirements for registration"@en-AU ;
    skos:narrower F2021L00308:35 ;
    skos:prefLabel "Part P36"@en-AU ;
    dcat:accessURL <https://www.legislation.gov.au/F2021L00308/2023-08-04/2023-08-04/text/original/epub/OEBPS/document_1/document_1.html#_Toc143604745> ;
    dcat:landingPage "https://www.legislation.gov.au/F2021L00308/2023-08-04/2023-08-04/text/original/epub/OEBPS/document_1/document_1.html#_Toc143604745"^^xsd:anyURI ;
    dcat:theme legcons:Part .

F2021L00308:188 a legcons:Division,
        owl:Class,
        dcat:Resource ;
    rdfs:label "Division - D188 Division 2 General rules relating to official marks"@en-AU ;
    dct:hasPart F2021L00308:189,
        F2021L00308:190,
        F2021L00308:191,
        F2021L00308:192,
        F2021L00308:193,
        F2021L00308:194,
        F2021L00308:195,
        F2021L00308:196,
        F2021L00308:197,
        F2021L00308:198,
        F2021L00308:199,
        F2021L00308:200 ;
    dct:isPartOf F2021L00308:176 ;
    dct:isReferencedBy F2021L00308: ;
    rdfs:comment "Division 2 General rules relating to official marks - Abrievated Graph Key: D188"@en-AU ;
    skos:broader F2021L00308:189,
        F2021L00308:190,
        F2021L00308:191,
        F2021L00308:192,
        F2021L00308:193,
        F2021L00308:194,
        F2021L00308:195,
        F2021L00308:196,
        F2021L00308:197,
        F2021L00308:198,
        F2021L00308:199,
        F2021L00308:200 ;
    skos:definition "Division 2 General rules relating to official marks"@en-AU ;
    skos:narrower F2021L00308:176 ;
    skos:prefLabel "Division D188"@en-AU ;
    dcat:accessURL <https://www.legislation.gov.au/F2021L00308/2023-08-04/2023-08-04/text/original/epub/OEBPS/document_1/document_1.html#_Toc143604897> ;
    dcat:landingPage "https://www.legislation.gov.au/F2021L00308/2023-08-04/2023-08-04/text/original/epub/OEBPS/document_1/document_1.html#_Toc143604897"^^xsd:anyURI ;
    dcat:theme legcons:Division .

F2021L00308:240 a legcons:Division,
        owl:Class,
        dcat:Resource ;
    rdfs:label "Division - D240 Division 2 Functions and powers"@en-AU ;
    dct:hasPart F2021L00308:241,
        F2021L00308:242,
        F2021L00308:243,
        F2021L00308:244,
        F2021L00308:245,
        F2021L00308:246,
        F2021L00308:247,
        F2021L00308:248,
        F2021L00308:249,
        F2021L00308:250,
        F2021L00308:251,
        F2021L00308:252,
        F2021L00308:253,
        F2021L00308:254,
        F2021L00308:255,
        F2021L00308:256 ;
    dct:isPartOf F2021L00308:237 ;
    dct:isReferencedBy F2021L00308: ;
    rdfs:comment "Division 2 Functions and powers - Abrievated Graph Key: D240"@en-AU ;
    skos:broader F2021L00308:241,
        F2021L00308:242,
        F2021L00308:243,
        F2021L00308:244,
        F2021L00308:245,
        F2021L00308:246,
        F2021L00308:247,
        F2021L00308:248,
        F2021L00308:249,
        F2021L00308:250,
        F2021L00308:251,
        F2021L00308:252,
        F2021L00308:253,
        F2021L00308:254,
        F2021L00308:255,
        F2021L00308:256 ;
    skos:definition "Division 2 Functions and powers"@en-AU ;
    skos:narrower F2021L00308:237 ;
    skos:prefLabel "Division D240"@en-AU ;
    dcat:accessURL <https://www.legislation.gov.au/F2021L00308/2023-08-04/2023-08-04/text/original/epub/OEBPS/document_1/document_1.html#_Toc143604949> ;
    dcat:landingPage "https://www.legislation.gov.au/F2021L00308/2023-08-04/2023-08-04/text/original/epub/OEBPS/document_1/document_1.html#_Toc143604949"^^xsd:anyURI ;
    dcat:theme legcons:Division .

F2021L00308:84 a legcons:Part,
        owl:Class,
        dcat:Resource ;
    rdfs:label "Part - P84 Part 2 Conditions of approved arrangement"@en-AU ;
    dct:hasPart F2021L00308:104,
        F2021L00308:105,
        F2021L00308:106,
        F2021L00308:107,
        F2021L00308:108,
        F2021L00308:109,
        F2021L00308:110,
        F2021L00308:111,
        F2021L00308:112,
        F2021L00308:116,
        F2021L00308:120,
        F2021L00308:121,
        F2021L00308:122,
        F2021L00308:123,
        F2021L00308:124,
        F2021L00308:125,
        F2021L00308:126,
        F2021L00308:127,
        F2021L00308:128,
        F2021L00308:129,
        F2021L00308:130,
        F2021L00308:131,
        F2021L00308:132,
        F2021L00308:133,
        F2021L00308:134,
        F2021L00308:135,
        F2021L00308:136,
        F2021L00308:137,
        F2021L00308:138,
        F2021L00308:139,
        F2021L00308:140,
        F2021L00308:141,
        F2021L00308:85,
        F2021L00308:87,
        F2021L00308:90 ;
    dct:isPartOf F2021L00308:80 ;
    dct:isReferencedBy F2021L00308: ;
    rdfs:comment "Part 2 Conditions of approved arrangement - Abrievated Graph Key: P84"@en-AU ;
    skos:broader F2021L00308:104,
        F2021L00308:105,
        F2021L00308:106,
        F2021L00308:107,
        F2021L00308:108,
        F2021L00308:109,
        F2021L00308:110,
        F2021L00308:111,
        F2021L00308:112,
        F2021L00308:116,
        F2021L00308:120,
        F2021L00308:121,
        F2021L00308:122,
        F2021L00308:123,
        F2021L00308:124,
        F2021L00308:125,
        F2021L00308:126,
        F2021L00308:127,
        F2021L00308:128,
        F2021L00308:129,
        F2021L00308:130,
        F2021L00308:131,
        F2021L00308:132,
        F2021L00308:133,
        F2021L00308:134,
        F2021L00308:135,
        F2021L00308:136,
        F2021L00308:137,
        F2021L00308:138,
        F2021L00308:139,
        F2021L00308:140,
        F2021L00308:141,
        F2021L00308:85,
        F2021L00308:87,
        F2021L00308:90 ;
    skos:definition "Part 2 Conditions of approved arrangement"@en-AU ;
    skos:narrower F2021L00308:80 ;
    skos:prefLabel "Part P84"@en-AU ;
    dcat:accessURL <https://www.legislation.gov.au/F2021L00308/2023-08-04/2023-08-04/text/original/epub/OEBPS/document_1/document_1.html#_Toc143604793> ;
    dcat:landingPage "https://www.legislation.gov.au/F2021L00308/2023-08-04/2023-08-04/text/original/epub/OEBPS/document_1/document_1.html#_Toc143604793"^^xsd:anyURI ;
    dcat:theme legcons:Part .

F2021L00308: a owl:Class,
        dcat:Dataset,
        dcat:Resource ;
    rdfs:label "Export Control (Rabbit and Ratite Meat and Rabbit and Ratite Meat Products) Rules 2021" ;
    dct:Jurisdiction " Department of Agriculture, Fisheries and Forestry "@en-AU ;
    dct:created "2024-08-30T15:14:22.818287"^^xsd:dateTime ;
    dct:creator "https://orcid.org/0009-0007-8434-7325"^^xsd:anyURI ;
    dct:date "2023-08-04T00:00:00+10:00"^^xsd:dateTime ;
    dct:description "Export Control (Rabbit and Ratite Meat and Rabbit and Ratite Meat Products) Rules 2021"@en-AU ;
    dct:identifier "https://www.legislation.gov.au/F2021L00308/latest"^^xsd:anyURI ;
    dct:license <https://creativecommons.org/licenses/by-sa/4.0/> ;
    dct:source "scheme=AGLSTERMS.AglsAgent; corporateName=Office Parliamentary Counsel; address=Locked Bag 30 Kingston ACT 2604; contact=+61 2 6120 1400"@en-AU ;
    dct:subject "Export Control (Rabbit and Ratite Meat and Rabbit and Ratite Meat Products) Rules 2021"@en-AU ;
    dct:title "Export Control (Rabbit and Ratite Meat and Rabbit and Ratite Meat Products) Rules 2021"@en-AU ;
    owl:imports legcons: ;
    dcat:theme legcons:Chapter,
        legcons:Division,
        legcons:Endnotes,
        legcons:Item,
        legcons:Part,
        legcons:Schedule,
        legcons:Subdivision ;
    schema:identifier "F2021L00308" ;
    schema:status "In force" ;
    schema:version "F2023C00741 (C03)" .

