@prefix : <http://example.org/au/leg/concepts/> .
@prefix leg: <http://example.org/au/leg/concepts/> .
@prefix dcterms: <http://purl.org/dc/terms/> .
@prefix owl: <http://www.w3.org/2002/07/owl#> .
@prefix prov: <http://www.w3.org/ns/prov#> .
@prefix rdf: <http://www.w3.org/1999/02/22-rdf-syntax-ns#> .
@prefix rdfs: <http://www.w3.org/2000/01/rdf-schema#> .
@prefix sdo: <http://schema.org#> .
@prefix skos: <http://www.w3.org/2004/02/skos/core#> .
@prefix xsd: <http://www.w3.org/2001/XMLSchema#> .

:leg a owl:Ontology, skos:ConceptScheme ;
    owl:versionIRI :0.1 ;
    owl:versionInfo "0.1" ;
    dcterms:title "Legilsation Concepts for Australilan Statutes" ;
    dcterms:identifier "https://www.legislation.gov.au" ;
    dcterms:creator <https://orcid.org/0009-0007-8434-7325> ;
    dcterms:publisher <https://orcid.org/0009-0007-8434-7325> ;
    dcterms:description "A SKOS Concept Scheme for Legislation/Statute Components" ;
    sdo:dateCreated "2024-07-29"^^xsd:date ;
    sdo:dateModified "2024-07-29"^^xsd:date ;
    dcterms:language dcterms:RFC4646:en-AU ;
    skos:hasTopConcept
		:chapter ;
	skos:prefLabel "Legilsation Concepts for Australilan Statutes"@en
.

<https://orcid.org/0009-0007-8434-7325>
    a sdo:Person ;
    sdo:affiliation <https://uncefact.github.io/spec-untp/> ;
    sdo:email "seewodg@gmail.com"^^xsd:anyURI ;
    sdo:name "Marcus Jowsey" ;
    sdo:url "https://www.linkedin.com/in/marcus-jowsey-surround/"^^xsd:anyURI ;
	skos:prefLabel "0009-0007-8434-7325"@en
.

<https://uncefact.github.io/spec-untp/>
    a sdo:Organization ;
    sdo:name "United Nations Transparency Protocol" ;
    sdo:url "https://uncefact.github.io/spec-untp/"^^xsd:anyURI ;
	skos:prefLabel "UNTP"@en
.

:chapter
    a skos:Concept , owl:Class ;
    skos:definition "The component of a regulation/statute that is a top level component."@en ;
    skos:inScheme :leg ;
    skos:prefLabel "Chapter"@en ;
    skos:topConceptOf :leg ;
	rdfs:subClassOf :leg ;
	skos:hasTopConcept :part ;
    schema:citation "https://www.legislation.gov.au/help-and-resources/understanding-legislation/structure-of-a-law"^^xsd:anyURI 
.

:part
    a skos:Concept , owl:Class ;
    skos:definition "The component of a regulation/statute that is component under chapter."@en ;
    skos:inScheme :leg ;
    skos:prefLabel "Part"@en ;
    skos:topConceptOf :chapter ;
	rdfs:subClassOf :chapter ;
	skos:hasTopConcept :division ;
    schema:citation "https://www.legislation.gov.au/help-and-resources/understanding-legislation/structure-of-a-law"^^xsd:anyURI 
.

:division
    a skos:Concept , owl:Class ;
    skos:definition "The component of a regulation/statute that is component under part."@en ;
    skos:inScheme :leg ;
    skos:prefLabel "Division"@en ;
    skos:topConceptOf :part ;
	rdfs:subClassOf :part ;
	skos:hasTopConcept :subdivision ;
    schema:citation "https://www.legislation.gov.au/help-and-resources/understanding-legislation/structure-of-a-law"^^xsd:anyURI ;
.

:subdivision
    a skos:Concept , owl:Class ;
    skos:definition "The component of a regulation/statute that is component under division."@en ;
    skos:inScheme :leg ;
    skos:prefLabel "Subdivision"@en ;
    skos:topConceptOf :division ;
	rdfs:subClassOf :division ;
    schema:citation "https://www.legislation.gov.au/help-and-resources/understanding-legislation/structure-of-a-law"^^xsd:anyURI ;
.